<?xml version="1.0" encoding="UTF-8"?>
<rdf:RDF
  xmlns:rdf="http://www.w3.org/1999/02/22-rdf-syntax-ns#"
  xmlns:rdfs="http://www.w3.org/2000/01/rdf-schema#"
  xmlns:owl="http://www.w3.org/2002/07/owl#"
  xmlns:xsd="http://www.w3.org/2001/XMLSchema#"
  xml:base="http://example.org/onto/">
  <owl:Class rdf:about="http://example.org/onto/class/aws_timestreaminfluxdb_db_instance">
    <rdfs:label>aws_timestreaminfluxdb_db_instance</rdfs:label>
    <rdfs:comment>Terraform resource for managing an Amazon Timestream for InfluxDB database instance.</rdfs:comment>
  </owl:Class>
  <owl:DatatypeProperty rdf:about="http://example.org/onto/prop/aws_timestreaminfluxdb_db_instance_allocated_storage">
    <rdfs:label>allocated_storage</rdfs:label>
    <rdfs:comment>The amount of storage to allocate for your DB storage type in GiB (gibibytes).</rdfs:comment>
    <rdfs:domain rdf:resource="http://example.org/onto/class/aws_timestreaminfluxdb_db_instance"/>
    <rdfs:range rdf:resource="http://www.w3.org/2001/XMLSchema#string"/>
  </owl:DatatypeProperty>
  <owl:DatatypeProperty rdf:about="http://example.org/onto/prop/aws_timestreaminfluxdb_db_instance_arn">
    <rdfs:label>arn</rdfs:label>
    <rdfs:domain rdf:resource="http://example.org/onto/class/aws_timestreaminfluxdb_db_instance"/>
    <rdfs:range rdf:resource="http://www.w3.org/2001/XMLSchema#string"/>
  </owl:DatatypeProperty>
  <owl:DatatypeProperty rdf:about="http://example.org/onto/prop/aws_timestreaminfluxdb_db_instance_availability_zone">
    <rdfs:label>availability_zone</rdfs:label>
    <rdfs:comment>The Availability Zone in which the DB instance resides.</rdfs:comment>
    <rdfs:domain rdf:resource="http://example.org/onto/class/aws_timestreaminfluxdb_db_instance"/>
    <rdfs:range rdf:resource="http://www.w3.org/2001/XMLSchema#string"/>
  </owl:DatatypeProperty>
  <owl:DatatypeProperty rdf:about="http://example.org/onto/prop/aws_timestreaminfluxdb_db_instance_bucket">
    <rdfs:label>bucket</rdfs:label>
    <rdfs:comment>The name of the initial InfluxDB bucket. All InfluxDB data is stored in a bucket. 
					A bucket combines the concept of a database and a retention period (the duration of time 
					that each data point persists). A bucket belongs to an organization.</rdfs:comment>
    <rdfs:domain rdf:resource="http://example.org/onto/class/aws_timestreaminfluxdb_db_instance"/>
    <rdfs:range rdf:resource="http://www.w3.org/2001/XMLSchema#string"/>
  </owl:DatatypeProperty>
  <owl:DatatypeProperty rdf:about="http://example.org/onto/prop/aws_timestreaminfluxdb_db_instance_db_instance_type">
    <rdfs:label>db_instance_type</rdfs:label>
    <rdfs:comment>The Timestream for InfluxDB DB instance type to run InfluxDB on.</rdfs:comment>
    <rdfs:domain rdf:resource="http://example.org/onto/class/aws_timestreaminfluxdb_db_instance"/>
    <rdfs:range rdf:resource="http://www.w3.org/2001/XMLSchema#string"/>
  </owl:DatatypeProperty>
  <owl:DatatypeProperty rdf:about="http://example.org/onto/prop/aws_timestreaminfluxdb_db_instance_db_parameter_group_identifier">
    <rdfs:label>db_parameter_group_identifier</rdfs:label>
    <rdfs:comment>The id of the DB parameter group assigned to your DB instance.</rdfs:comment>
    <rdfs:domain rdf:resource="http://example.org/onto/class/aws_timestreaminfluxdb_db_instance"/>
    <rdfs:range rdf:resource="http://www.w3.org/2001/XMLSchema#string"/>
  </owl:DatatypeProperty>
  <owl:DatatypeProperty rdf:about="http://example.org/onto/prop/aws_timestreaminfluxdb_db_instance_db_storage_type">
    <rdfs:label>db_storage_type</rdfs:label>
    <rdfs:comment>The Timestream for InfluxDB DB storage type to read and write InfluxDB data. 
					You can choose between 3 different types of provisioned Influx IOPS included storage according 
					to your workloads requirements: Influx IO Included 3000 IOPS, Influx IO Included 12000 IOPS, 
					Influx IO Included 16000 IOPS.</rdfs:comment>
    <rdfs:domain rdf:resource="http://example.org/onto/class/aws_timestreaminfluxdb_db_instance"/>
    <rdfs:range rdf:resource="http://www.w3.org/2001/XMLSchema#string"/>
  </owl:DatatypeProperty>
  <owl:DatatypeProperty rdf:about="http://example.org/onto/prop/aws_timestreaminfluxdb_db_instance_deployment_type">
    <rdfs:label>deployment_type</rdfs:label>
    <rdfs:comment>Specifies whether the DB instance will be deployed as a standalone instance or 
					with a Multi-AZ standby for high availability.</rdfs:comment>
    <rdfs:domain rdf:resource="http://example.org/onto/class/aws_timestreaminfluxdb_db_instance"/>
    <rdfs:range rdf:resource="http://www.w3.org/2001/XMLSchema#string"/>
  </owl:DatatypeProperty>
  <owl:DatatypeProperty rdf:about="http://example.org/onto/prop/aws_timestreaminfluxdb_db_instance_endpoint">
    <rdfs:label>endpoint</rdfs:label>
    <rdfs:comment>The endpoint used to connect to InfluxDB. The default InfluxDB port is 8086.</rdfs:comment>
    <rdfs:domain rdf:resource="http://example.org/onto/class/aws_timestreaminfluxdb_db_instance"/>
    <rdfs:range rdf:resource="http://www.w3.org/2001/XMLSchema#string"/>
  </owl:DatatypeProperty>
  <owl:DatatypeProperty rdf:about="http://example.org/onto/prop/aws_timestreaminfluxdb_db_instance_id">
    <rdfs:label>id</rdfs:label>
    <rdfs:domain rdf:resource="http://example.org/onto/class/aws_timestreaminfluxdb_db_instance"/>
    <rdfs:range rdf:resource="http://www.w3.org/2001/XMLSchema#string"/>
  </owl:DatatypeProperty>
  <owl:DatatypeProperty rdf:about="http://example.org/onto/prop/aws_timestreaminfluxdb_db_instance_influx_auth_parameters_secret_arn">
    <rdfs:label>influx_auth_parameters_secret_arn</rdfs:label>
    <rdfs:comment>The Amazon Resource Name (ARN) of the AWS Secrets Manager secret containing the 
					initial InfluxDB authorization parameters. The secret value is a JSON formatted 
					key-value pair holding InfluxDB authorization values: organization, bucket, 
					username, and password.</rdfs:comment>
    <rdfs:domain rdf:resource="http://example.org/onto/class/aws_timestreaminfluxdb_db_instance"/>
    <rdfs:range rdf:resource="http://www.w3.org/2001/XMLSchema#string"/>
  </owl:DatatypeProperty>
  <owl:DatatypeProperty rdf:about="http://example.org/onto/prop/aws_timestreaminfluxdb_db_instance_name">
    <rdfs:label>name</rdfs:label>
    <rdfs:comment>The name that uniquely identifies the DB instance when interacting with the 
					Amazon Timestream for InfluxDB API and CLI commands. This name will also be a 
					prefix included in the endpoint. DB instance names must be unique per customer 
					and per region.</rdfs:comment>
    <rdfs:domain rdf:resource="http://example.org/onto/class/aws_timestreaminfluxdb_db_instance"/>
    <rdfs:range rdf:resource="http://www.w3.org/2001/XMLSchema#string"/>
  </owl:DatatypeProperty>
  <owl:DatatypeProperty rdf:about="http://example.org/onto/prop/aws_timestreaminfluxdb_db_instance_network_type">
    <rdfs:label>network_type</rdfs:label>
    <rdfs:comment>Specifies whether the networkType of the Timestream for InfluxDB instance is 
					IPV4, which can communicate over IPv4 protocol only, or DUAL, which can communicate 
					over both IPv4 and IPv6 protocols.</rdfs:comment>
    <rdfs:domain rdf:resource="http://example.org/onto/class/aws_timestreaminfluxdb_db_instance"/>
    <rdfs:range rdf:resource="http://www.w3.org/2001/XMLSchema#string"/>
  </owl:DatatypeProperty>
  <owl:DatatypeProperty rdf:about="http://example.org/onto/prop/aws_timestreaminfluxdb_db_instance_organization">
    <rdfs:label>organization</rdfs:label>
    <rdfs:comment>The name of the initial organization for the initial admin user in InfluxDB. An 
					InfluxDB organization is a workspace for a group of users.</rdfs:comment>
    <rdfs:domain rdf:resource="http://example.org/onto/class/aws_timestreaminfluxdb_db_instance"/>
    <rdfs:range rdf:resource="http://www.w3.org/2001/XMLSchema#string"/>
  </owl:DatatypeProperty>
  <owl:DatatypeProperty rdf:about="http://example.org/onto/prop/aws_timestreaminfluxdb_db_instance_password">
    <rdfs:label>password</rdfs:label>
    <rdfs:comment>The password of the initial admin user created in InfluxDB. This password will 
					allow you to access the InfluxDB UI to perform various administrative tasks and 
					also use the InfluxDB CLI to create an operator token. These attributes will be 
					stored in a Secret created in AWS SecretManager in your account.</rdfs:comment>
    <rdfs:domain rdf:resource="http://example.org/onto/class/aws_timestreaminfluxdb_db_instance"/>
    <rdfs:range rdf:resource="http://www.w3.org/2001/XMLSchema#string"/>
  </owl:DatatypeProperty>
  <owl:DatatypeProperty rdf:about="http://example.org/onto/prop/aws_timestreaminfluxdb_db_instance_port">
    <rdfs:label>port</rdfs:label>
    <rdfs:comment>The port number on which InfluxDB accepts connections.</rdfs:comment>
    <rdfs:domain rdf:resource="http://example.org/onto/class/aws_timestreaminfluxdb_db_instance"/>
    <rdfs:range rdf:resource="http://www.w3.org/2001/XMLSchema#string"/>
  </owl:DatatypeProperty>
  <owl:DatatypeProperty rdf:about="http://example.org/onto/prop/aws_timestreaminfluxdb_db_instance_publicly_accessible">
    <rdfs:label>publicly_accessible</rdfs:label>
    <rdfs:comment>Configures the DB instance with a public IP to facilitate access.</rdfs:comment>
    <rdfs:domain rdf:resource="http://example.org/onto/class/aws_timestreaminfluxdb_db_instance"/>
    <rdfs:range rdf:resource="http://www.w3.org/2001/XMLSchema#string"/>
  </owl:DatatypeProperty>
  <owl:DatatypeProperty rdf:about="http://example.org/onto/prop/aws_timestreaminfluxdb_db_instance_region">
    <rdfs:label>region</rdfs:label>
    <rdfs:comment>Region where this resource will be [managed](https://docs.aws.amazon.com/general/latest/gr/rande.html#regional-endpoints). Defaults to the Region set in the [provider configuration](https://registry.terraform.io/providers/hashicorp/aws/latest/docs#aws-configuration-reference).</rdfs:comment>
    <rdfs:domain rdf:resource="http://example.org/onto/class/aws_timestreaminfluxdb_db_instance"/>
    <rdfs:range rdf:resource="http://www.w3.org/2001/XMLSchema#string"/>
  </owl:DatatypeProperty>
  <owl:DatatypeProperty rdf:about="http://example.org/onto/prop/aws_timestreaminfluxdb_db_instance_secondary_availability_zone">
    <rdfs:label>secondary_availability_zone</rdfs:label>
    <rdfs:comment>The Availability Zone in which the standby instance is located when deploying 
					with a MultiAZ standby instance.</rdfs:comment>
    <rdfs:domain rdf:resource="http://example.org/onto/class/aws_timestreaminfluxdb_db_instance"/>
    <rdfs:range rdf:resource="http://www.w3.org/2001/XMLSchema#string"/>
  </owl:DatatypeProperty>
  <owl:DatatypeProperty rdf:about="http://example.org/onto/prop/aws_timestreaminfluxdb_db_instance_tags">
    <rdfs:label>tags</rdfs:label>
    <rdfs:domain rdf:resource="http://example.org/onto/class/aws_timestreaminfluxdb_db_instance"/>
    <rdfs:range rdf:resource="http://www.w3.org/2001/XMLSchema#string"/>
  </owl:DatatypeProperty>
  <owl:DatatypeProperty rdf:about="http://example.org/onto/prop/aws_timestreaminfluxdb_db_instance_tags_all">
    <rdfs:label>tags_all</rdfs:label>
    <rdfs:domain rdf:resource="http://example.org/onto/class/aws_timestreaminfluxdb_db_instance"/>
    <rdfs:range rdf:resource="http://www.w3.org/2001/XMLSchema#string"/>
  </owl:DatatypeProperty>
  <owl:DatatypeProperty rdf:about="http://example.org/onto/prop/aws_timestreaminfluxdb_db_instance_username">
    <rdfs:label>username</rdfs:label>
    <rdfs:comment>The username of the initial admin user created in InfluxDB. 
					Must start with a letter and can't end with a hyphen or contain two 
					consecutive hyphens. For example, my-user1. This username will allow 
					you to access the InfluxDB UI to perform various administrative tasks 
					and also use the InfluxDB CLI to create an operator token. These 
					attributes will be stored in a Secret created in Amazon Secrets 
					Manager in your account</rdfs:comment>
    <rdfs:domain rdf:resource="http://example.org/onto/class/aws_timestreaminfluxdb_db_instance"/>
    <rdfs:range rdf:resource="http://www.w3.org/2001/XMLSchema#string"/>
  </owl:DatatypeProperty>
  <owl:DatatypeProperty rdf:about="http://example.org/onto/prop/aws_timestreaminfluxdb_db_instance_vpc_security_group_ids">
    <rdfs:label>vpc_security_group_ids</rdfs:label>
    <rdfs:comment>A list of VPC security group IDs to associate with the DB instance.</rdfs:comment>
    <rdfs:domain rdf:resource="http://example.org/onto/class/aws_timestreaminfluxdb_db_instance"/>
    <rdfs:range rdf:resource="http://www.w3.org/2001/XMLSchema#string"/>
  </owl:DatatypeProperty>
  <owl:DatatypeProperty rdf:about="http://example.org/onto/prop/aws_timestreaminfluxdb_db_instance_vpc_subnet_ids">
    <rdfs:label>vpc_subnet_ids</rdfs:label>
    <rdfs:comment>A list of VPC subnet IDs to associate with the DB instance. Provide at least 
					two VPC subnet IDs in different availability zones when deploying with a Multi-AZ standby.</rdfs:comment>
    <rdfs:domain rdf:resource="http://example.org/onto/class/aws_timestreaminfluxdb_db_instance"/>
    <rdfs:range rdf:resource="http://www.w3.org/2001/XMLSchema#string"/>
  </owl:DatatypeProperty>
  <owl:DatatypeProperty rdf:about="http://example.org/onto/prop/aws_timestreaminfluxdb_db_instance_bucket_name">
    <rdfs:label>bucket_name</rdfs:label>
    <rdfs:comment>The name of the S3 bucket to deliver logs to.</rdfs:comment>
    <rdfs:domain rdf:resource="http://example.org/onto/class/aws_timestreaminfluxdb_db_instance"/>
    <rdfs:range rdf:resource="http://www.w3.org/2001/XMLSchema#string"/>
  </owl:DatatypeProperty>
  <owl:DatatypeProperty rdf:about="http://example.org/onto/prop/aws_timestreaminfluxdb_db_instance_enabled">
    <rdfs:label>enabled</rdfs:label>
    <rdfs:comment>Indicates whether log delivery to the S3 bucket is enabled.</rdfs:comment>
    <rdfs:domain rdf:resource="http://example.org/onto/class/aws_timestreaminfluxdb_db_instance"/>
    <rdfs:range rdf:resource="http://www.w3.org/2001/XMLSchema#string"/>
  </owl:DatatypeProperty>
  <owl:DatatypeProperty rdf:about="http://example.org/onto/prop/aws_timestreaminfluxdb_db_instance_create">
    <rdfs:label>create</rdfs:label>
    <rdfs:comment>A string that can be [parsed as a duration](https://pkg.go.dev/time#ParseDuration) consisting of numbers and unit suffixes, such as "30s" or "2h45m". Valid time units are "s" (seconds), "m" (minutes), "h" (hours).</rdfs:comment>
    <rdfs:domain rdf:resource="http://example.org/onto/class/aws_timestreaminfluxdb_db_instance"/>
    <rdfs:range rdf:resource="http://www.w3.org/2001/XMLSchema#string"/>
  </owl:DatatypeProperty>
  <owl:DatatypeProperty rdf:about="http://example.org/onto/prop/aws_timestreaminfluxdb_db_instance_delete">
    <rdfs:label>delete</rdfs:label>
    <rdfs:comment>A string that can be [parsed as a duration](https://pkg.go.dev/time#ParseDuration) consisting of numbers and unit suffixes, such as "30s" or "2h45m". Valid time units are "s" (seconds), "m" (minutes), "h" (hours). Setting a timeout for a Delete operation is only applicable if changes are saved into state before the destroy operation occurs.</rdfs:comment>
    <rdfs:domain rdf:resource="http://example.org/onto/class/aws_timestreaminfluxdb_db_instance"/>
    <rdfs:range rdf:resource="http://www.w3.org/2001/XMLSchema#string"/>
  </owl:DatatypeProperty>
  <owl:DatatypeProperty rdf:about="http://example.org/onto/prop/aws_timestreaminfluxdb_db_instance_update">
    <rdfs:label>update</rdfs:label>
    <rdfs:comment>A string that can be [parsed as a duration](https://pkg.go.dev/time#ParseDuration) consisting of numbers and unit suffixes, such as "30s" or "2h45m". Valid time units are "s" (seconds), "m" (minutes), "h" (hours).</rdfs:comment>
    <rdfs:domain rdf:resource="http://example.org/onto/class/aws_timestreaminfluxdb_db_instance"/>
    <rdfs:range rdf:resource="http://www.w3.org/2001/XMLSchema#string"/>
  </owl:DatatypeProperty>
</rdf:RDF>
