<?xml version="1.0" encoding="UTF-8"?>
<rdf:RDF
  xmlns:rdf="http://www.w3.org/1999/02/22-rdf-syntax-ns#"
  xmlns:rdfs="http://www.w3.org/2000/01/rdf-schema#"
  xmlns:owl="http://www.w3.org/2002/07/owl#"
  xmlns:xsd="http://www.w3.org/2001/XMLSchema#"
  xml:base="http://example.org/onto/">
  <owl:Class rdf:about="http://example.org/onto/class/aws_dsql_cluster_peering">
    <rdfs:label>aws_dsql_cluster_peering</rdfs:label>
    <rdfs:comment>Terraform resource for managing an Amazon Aurora DSQL Cluster Peering.</rdfs:comment>
  </owl:Class>
  <owl:DatatypeProperty rdf:about="http://example.org/onto/prop/aws_dsql_cluster_peering_clusters">
    <rdfs:label>clusters</rdfs:label>
    <rdfs:domain rdf:resource="http://example.org/onto/class/aws_dsql_cluster_peering"/>
    <rdfs:range rdf:resource="http://www.w3.org/2001/XMLSchema#string"/>
  </owl:DatatypeProperty>
  <owl:DatatypeProperty rdf:about="http://example.org/onto/prop/aws_dsql_cluster_peering_identifier">
    <rdfs:label>identifier</rdfs:label>
    <rdfs:domain rdf:resource="http://example.org/onto/class/aws_dsql_cluster_peering"/>
    <rdfs:range rdf:resource="http://www.w3.org/2001/XMLSchema#string"/>
  </owl:DatatypeProperty>
  <owl:DatatypeProperty rdf:about="http://example.org/onto/prop/aws_dsql_cluster_peering_region">
    <rdfs:label>region</rdfs:label>
    <rdfs:comment>Region where this resource will be [managed](https://docs.aws.amazon.com/general/latest/gr/rande.html#regional-endpoints). Defaults to the Region set in the [provider configuration](https://registry.terraform.io/providers/hashicorp/aws/latest/docs#aws-configuration-reference).</rdfs:comment>
    <rdfs:domain rdf:resource="http://example.org/onto/class/aws_dsql_cluster_peering"/>
    <rdfs:range rdf:resource="http://www.w3.org/2001/XMLSchema#string"/>
  </owl:DatatypeProperty>
  <owl:DatatypeProperty rdf:about="http://example.org/onto/prop/aws_dsql_cluster_peering_witness_region">
    <rdfs:label>witness_region</rdfs:label>
    <rdfs:domain rdf:resource="http://example.org/onto/class/aws_dsql_cluster_peering"/>
    <rdfs:range rdf:resource="http://www.w3.org/2001/XMLSchema#string"/>
  </owl:DatatypeProperty>
  <owl:DatatypeProperty rdf:about="http://example.org/onto/prop/aws_dsql_cluster_peering_create">
    <rdfs:label>create</rdfs:label>
    <rdfs:comment>A string that can be [parsed as a duration](https://pkg.go.dev/time#ParseDuration) consisting of numbers and unit suffixes, such as "30s" or "2h45m". Valid time units are "s" (seconds), "m" (minutes), "h" (hours).</rdfs:comment>
    <rdfs:domain rdf:resource="http://example.org/onto/class/aws_dsql_cluster_peering"/>
    <rdfs:range rdf:resource="http://www.w3.org/2001/XMLSchema#string"/>
  </owl:DatatypeProperty>
</rdf:RDF>
