<?xml version="1.0" encoding="UTF-8"?>
<rdf:RDF
  xmlns:rdf="http://www.w3.org/1999/02/22-rdf-syntax-ns#"
  xmlns:rdfs="http://www.w3.org/2000/01/rdf-schema#"
  xmlns:owl="http://www.w3.org/2002/07/owl#"
  xmlns:xsd="http://www.w3.org/2001/XMLSchema#"
  xml:base="http://example.org/onto/">
  <owl:Class rdf:about="http://example.org/onto/class/aws_odb_network">
    <rdfs:label>aws_odb_network</rdfs:label>
    <rdfs:comment>Terraform resource for managing odb Network resource in AWS for Oracle Database@AWS.</rdfs:comment>
  </owl:Class>
  <owl:DatatypeProperty rdf:about="http://example.org/onto/prop/aws_odb_network_arn">
    <rdfs:label>arn</rdfs:label>
    <rdfs:domain rdf:resource="http://example.org/onto/class/aws_odb_network"/>
    <rdfs:range rdf:resource="http://www.w3.org/2001/XMLSchema#string"/>
  </owl:DatatypeProperty>
  <owl:DatatypeProperty rdf:about="http://example.org/onto/prop/aws_odb_network_availability_zone">
    <rdfs:label>availability_zone</rdfs:label>
    <rdfs:comment>The name of the Availability Zone (AZ) where the odb network is located. Changing this will force terraform to create new resource</rdfs:comment>
    <rdfs:domain rdf:resource="http://example.org/onto/class/aws_odb_network"/>
    <rdfs:range rdf:resource="http://www.w3.org/2001/XMLSchema#string"/>
  </owl:DatatypeProperty>
  <owl:DatatypeProperty rdf:about="http://example.org/onto/prop/aws_odb_network_availability_zone_id">
    <rdfs:label>availability_zone_id</rdfs:label>
    <rdfs:comment>The AZ ID of the AZ where the ODB network is located. Changing this will force terraform to create new resource.</rdfs:comment>
    <rdfs:domain rdf:resource="http://example.org/onto/class/aws_odb_network"/>
    <rdfs:range rdf:resource="http://www.w3.org/2001/XMLSchema#string"/>
  </owl:DatatypeProperty>
  <owl:DatatypeProperty rdf:about="http://example.org/onto/prop/aws_odb_network_backup_subnet_cidr">
    <rdfs:label>backup_subnet_cidr</rdfs:label>
    <rdfs:comment>The CIDR range of the backup subnet for the ODB network. Changing this will force terraform to create new resource.
	Constraints:
	   - Must not overlap with the CIDR range of the client subnet.
	   - Must not overlap with the CIDR ranges of the VPCs that are connected to the
	   ODB network.
	   - Must not use the following CIDR ranges that are reserved by OCI:
	   - 100.106.0.0/16 and 100.107.0.0/16
	   - 169.254.0.0/16
	   - 224.0.0.0 - 239.255.255.255
	   - 240.0.0.0 - 255.255.255.255</rdfs:comment>
    <rdfs:domain rdf:resource="http://example.org/onto/class/aws_odb_network"/>
    <rdfs:range rdf:resource="http://www.w3.org/2001/XMLSchema#string"/>
  </owl:DatatypeProperty>
  <owl:DatatypeProperty rdf:about="http://example.org/onto/prop/aws_odb_network_client_subnet_cidr">
    <rdfs:label>client_subnet_cidr</rdfs:label>
    <rdfs:comment>The CIDR notation for the network resource. Changing this will force terraform to create new resource.
 Constraints:
  	 - Must not overlap with the CIDR range of the backup subnet.
   	- Must not overlap with the CIDR ranges of the VPCs that are connected to the
   ODB network.
  	- Must not use the following CIDR ranges that are reserved by OCI:
  	 - 100.106.0.0/16 and 100.107.0.0/16
  	 - 169.254.0.0/16
   	- 224.0.0.0 - 239.255.255.255
   	- 240.0.0.0 - 255.255.255.255</rdfs:comment>
    <rdfs:domain rdf:resource="http://example.org/onto/class/aws_odb_network"/>
    <rdfs:range rdf:resource="http://www.w3.org/2001/XMLSchema#string"/>
  </owl:DatatypeProperty>
  <owl:DatatypeProperty rdf:about="http://example.org/onto/prop/aws_odb_network_created_at">
    <rdfs:label>created_at</rdfs:label>
    <rdfs:comment>The date and time when the ODB network was created.</rdfs:comment>
    <rdfs:domain rdf:resource="http://example.org/onto/class/aws_odb_network"/>
    <rdfs:range rdf:resource="http://www.w3.org/2001/XMLSchema#string"/>
  </owl:DatatypeProperty>
  <owl:DatatypeProperty rdf:about="http://example.org/onto/prop/aws_odb_network_custom_domain_name">
    <rdfs:label>custom_domain_name</rdfs:label>
    <rdfs:comment>The name of the custom domain that the network is located. custom_domain_name and default_dns_prefix both can't be given.</rdfs:comment>
    <rdfs:domain rdf:resource="http://example.org/onto/class/aws_odb_network"/>
    <rdfs:range rdf:resource="http://www.w3.org/2001/XMLSchema#string"/>
  </owl:DatatypeProperty>
  <owl:DatatypeProperty rdf:about="http://example.org/onto/prop/aws_odb_network_default_dns_prefix">
    <rdfs:label>default_dns_prefix</rdfs:label>
    <rdfs:comment>The default DNS prefix for the network resource. Changing this will force terraform to create new resource.</rdfs:comment>
    <rdfs:domain rdf:resource="http://example.org/onto/class/aws_odb_network"/>
    <rdfs:range rdf:resource="http://www.w3.org/2001/XMLSchema#string"/>
  </owl:DatatypeProperty>
  <owl:DatatypeProperty rdf:about="http://example.org/onto/prop/aws_odb_network_display_name">
    <rdfs:label>display_name</rdfs:label>
    <rdfs:comment>The user-friendly name for the odb network. Changing this will force terraform to create a new resource.</rdfs:comment>
    <rdfs:domain rdf:resource="http://example.org/onto/class/aws_odb_network"/>
    <rdfs:range rdf:resource="http://www.w3.org/2001/XMLSchema#string"/>
  </owl:DatatypeProperty>
  <owl:DatatypeProperty rdf:about="http://example.org/onto/prop/aws_odb_network_id">
    <rdfs:label>id</rdfs:label>
    <rdfs:domain rdf:resource="http://example.org/onto/class/aws_odb_network"/>
    <rdfs:range rdf:resource="http://www.w3.org/2001/XMLSchema#string"/>
  </owl:DatatypeProperty>
  <owl:DatatypeProperty rdf:about="http://example.org/onto/prop/aws_odb_network_managed_services">
    <rdfs:label>managed_services</rdfs:label>
    <rdfs:comment>The managed services configuration for the ODB network.</rdfs:comment>
    <rdfs:domain rdf:resource="http://example.org/onto/class/aws_odb_network"/>
    <rdfs:range rdf:resource="http://www.w3.org/2001/XMLSchema#string"/>
  </owl:DatatypeProperty>
  <owl:DatatypeProperty rdf:about="http://example.org/onto/prop/aws_odb_network_oci_dns_forwarding_configs">
    <rdfs:label>oci_dns_forwarding_configs</rdfs:label>
    <rdfs:comment>The DNS resolver endpoint in OCI for forwarding DNS queries for the ociPrivateZone domain.</rdfs:comment>
    <rdfs:domain rdf:resource="http://example.org/onto/class/aws_odb_network"/>
    <rdfs:range rdf:resource="http://www.w3.org/2001/XMLSchema#string"/>
  </owl:DatatypeProperty>
  <owl:DatatypeProperty rdf:about="http://example.org/onto/prop/aws_odb_network_oci_network_anchor_id">
    <rdfs:label>oci_network_anchor_id</rdfs:label>
    <rdfs:comment>The unique identifier of the OCI network anchor for the ODB network.</rdfs:comment>
    <rdfs:domain rdf:resource="http://example.org/onto/class/aws_odb_network"/>
    <rdfs:range rdf:resource="http://www.w3.org/2001/XMLSchema#string"/>
  </owl:DatatypeProperty>
  <owl:DatatypeProperty rdf:about="http://example.org/onto/prop/aws_odb_network_oci_network_anchor_url">
    <rdfs:label>oci_network_anchor_url</rdfs:label>
    <rdfs:comment>The URL of the OCI network anchor for the ODB network.</rdfs:comment>
    <rdfs:domain rdf:resource="http://example.org/onto/class/aws_odb_network"/>
    <rdfs:range rdf:resource="http://www.w3.org/2001/XMLSchema#string"/>
  </owl:DatatypeProperty>
  <owl:DatatypeProperty rdf:about="http://example.org/onto/prop/aws_odb_network_oci_resource_anchor_name">
    <rdfs:label>oci_resource_anchor_name</rdfs:label>
    <rdfs:comment>The name of the OCI resource anchor for the ODB network.</rdfs:comment>
    <rdfs:domain rdf:resource="http://example.org/onto/class/aws_odb_network"/>
    <rdfs:range rdf:resource="http://www.w3.org/2001/XMLSchema#string"/>
  </owl:DatatypeProperty>
  <owl:DatatypeProperty rdf:about="http://example.org/onto/prop/aws_odb_network_oci_vcn_id">
    <rdfs:label>oci_vcn_id</rdfs:label>
    <rdfs:comment>The unique identifier  Oracle Cloud ID (OCID) of the OCI VCN for the ODB network.</rdfs:comment>
    <rdfs:domain rdf:resource="http://example.org/onto/class/aws_odb_network"/>
    <rdfs:range rdf:resource="http://www.w3.org/2001/XMLSchema#string"/>
  </owl:DatatypeProperty>
  <owl:DatatypeProperty rdf:about="http://example.org/onto/prop/aws_odb_network_oci_vcn_url">
    <rdfs:label>oci_vcn_url</rdfs:label>
    <rdfs:comment>The URL of the OCI VCN for the ODB network.</rdfs:comment>
    <rdfs:domain rdf:resource="http://example.org/onto/class/aws_odb_network"/>
    <rdfs:range rdf:resource="http://www.w3.org/2001/XMLSchema#string"/>
  </owl:DatatypeProperty>
  <owl:DatatypeProperty rdf:about="http://example.org/onto/prop/aws_odb_network_peered_cidrs">
    <rdfs:label>peered_cidrs</rdfs:label>
    <rdfs:comment>The list of CIDR ranges from the peered VPC that are allowed access to the ODB network. Please refer odb network peering documentation.</rdfs:comment>
    <rdfs:domain rdf:resource="http://example.org/onto/class/aws_odb_network"/>
    <rdfs:range rdf:resource="http://www.w3.org/2001/XMLSchema#string"/>
  </owl:DatatypeProperty>
  <owl:DatatypeProperty rdf:about="http://example.org/onto/prop/aws_odb_network_percent_progress">
    <rdfs:label>percent_progress</rdfs:label>
    <rdfs:comment>The amount of progress made on the current operation on the ODB network, expressed as a percentage.</rdfs:comment>
    <rdfs:domain rdf:resource="http://example.org/onto/class/aws_odb_network"/>
    <rdfs:range rdf:resource="http://www.w3.org/2001/XMLSchema#string"/>
  </owl:DatatypeProperty>
  <owl:DatatypeProperty rdf:about="http://example.org/onto/prop/aws_odb_network_region">
    <rdfs:label>region</rdfs:label>
    <rdfs:comment>Region where this resource will be [managed](https://docs.aws.amazon.com/general/latest/gr/rande.html#regional-endpoints). Defaults to the Region set in the [provider configuration](https://registry.terraform.io/providers/hashicorp/aws/latest/docs#aws-configuration-reference).</rdfs:comment>
    <rdfs:domain rdf:resource="http://example.org/onto/class/aws_odb_network"/>
    <rdfs:range rdf:resource="http://www.w3.org/2001/XMLSchema#string"/>
  </owl:DatatypeProperty>
  <owl:DatatypeProperty rdf:about="http://example.org/onto/prop/aws_odb_network_s3_access">
    <rdfs:label>s3_access</rdfs:label>
    <rdfs:comment>Specifies the configuration for Amazon S3 access from the ODB network.</rdfs:comment>
    <rdfs:domain rdf:resource="http://example.org/onto/class/aws_odb_network"/>
    <rdfs:range rdf:resource="http://www.w3.org/2001/XMLSchema#string"/>
  </owl:DatatypeProperty>
  <owl:DatatypeProperty rdf:about="http://example.org/onto/prop/aws_odb_network_s3_policy_document">
    <rdfs:label>s3_policy_document</rdfs:label>
    <rdfs:comment>Specifies the endpoint policy for Amazon S3 access from the ODB network.</rdfs:comment>
    <rdfs:domain rdf:resource="http://example.org/onto/class/aws_odb_network"/>
    <rdfs:range rdf:resource="http://www.w3.org/2001/XMLSchema#string"/>
  </owl:DatatypeProperty>
  <owl:DatatypeProperty rdf:about="http://example.org/onto/prop/aws_odb_network_status">
    <rdfs:label>status</rdfs:label>
    <rdfs:comment>The status of the network resource.</rdfs:comment>
    <rdfs:domain rdf:resource="http://example.org/onto/class/aws_odb_network"/>
    <rdfs:range rdf:resource="http://www.w3.org/2001/XMLSchema#string"/>
  </owl:DatatypeProperty>
  <owl:DatatypeProperty rdf:about="http://example.org/onto/prop/aws_odb_network_status_reason">
    <rdfs:label>status_reason</rdfs:label>
    <rdfs:comment>Additional information about the current status of the ODB network.</rdfs:comment>
    <rdfs:domain rdf:resource="http://example.org/onto/class/aws_odb_network"/>
    <rdfs:range rdf:resource="http://www.w3.org/2001/XMLSchema#string"/>
  </owl:DatatypeProperty>
  <owl:DatatypeProperty rdf:about="http://example.org/onto/prop/aws_odb_network_tags">
    <rdfs:label>tags</rdfs:label>
    <rdfs:domain rdf:resource="http://example.org/onto/class/aws_odb_network"/>
    <rdfs:range rdf:resource="http://www.w3.org/2001/XMLSchema#string"/>
  </owl:DatatypeProperty>
  <owl:DatatypeProperty rdf:about="http://example.org/onto/prop/aws_odb_network_tags_all">
    <rdfs:label>tags_all</rdfs:label>
    <rdfs:domain rdf:resource="http://example.org/onto/class/aws_odb_network"/>
    <rdfs:range rdf:resource="http://www.w3.org/2001/XMLSchema#string"/>
  </owl:DatatypeProperty>
  <owl:DatatypeProperty rdf:about="http://example.org/onto/prop/aws_odb_network_zero_etl_access">
    <rdfs:label>zero_etl_access</rdfs:label>
    <rdfs:comment>Specifies the configuration for Zero-ETL access from the ODB network.</rdfs:comment>
    <rdfs:domain rdf:resource="http://example.org/onto/class/aws_odb_network"/>
    <rdfs:range rdf:resource="http://www.w3.org/2001/XMLSchema#string"/>
  </owl:DatatypeProperty>
  <owl:DatatypeProperty rdf:about="http://example.org/onto/prop/aws_odb_network_create">
    <rdfs:label>create</rdfs:label>
    <rdfs:comment>A string that can be [parsed as a duration](https://pkg.go.dev/time#ParseDuration) consisting of numbers and unit suffixes, such as "30s" or "2h45m". Valid time units are "s" (seconds), "m" (minutes), "h" (hours).</rdfs:comment>
    <rdfs:domain rdf:resource="http://example.org/onto/class/aws_odb_network"/>
    <rdfs:range rdf:resource="http://www.w3.org/2001/XMLSchema#string"/>
  </owl:DatatypeProperty>
  <owl:DatatypeProperty rdf:about="http://example.org/onto/prop/aws_odb_network_delete">
    <rdfs:label>delete</rdfs:label>
    <rdfs:comment>A string that can be [parsed as a duration](https://pkg.go.dev/time#ParseDuration) consisting of numbers and unit suffixes, such as "30s" or "2h45m". Valid time units are "s" (seconds), "m" (minutes), "h" (hours). Setting a timeout for a Delete operation is only applicable if changes are saved into state before the destroy operation occurs.</rdfs:comment>
    <rdfs:domain rdf:resource="http://example.org/onto/class/aws_odb_network"/>
    <rdfs:range rdf:resource="http://www.w3.org/2001/XMLSchema#string"/>
  </owl:DatatypeProperty>
  <owl:DatatypeProperty rdf:about="http://example.org/onto/prop/aws_odb_network_update">
    <rdfs:label>update</rdfs:label>
    <rdfs:comment>A string that can be [parsed as a duration](https://pkg.go.dev/time#ParseDuration) consisting of numbers and unit suffixes, such as "30s" or "2h45m". Valid time units are "s" (seconds), "m" (minutes), "h" (hours).</rdfs:comment>
    <rdfs:domain rdf:resource="http://example.org/onto/class/aws_odb_network"/>
    <rdfs:range rdf:resource="http://www.w3.org/2001/XMLSchema#string"/>
  </owl:DatatypeProperty>
</rdf:RDF>
