<?xml version="1.0" encoding="UTF-8"?>
<rdf:RDF
  xmlns:rdf="http://www.w3.org/1999/02/22-rdf-syntax-ns#"
  xmlns:rdfs="http://www.w3.org/2000/01/rdf-schema#"
  xmlns:owl="http://www.w3.org/2002/07/owl#"
  xmlns:xsd="http://www.w3.org/2001/XMLSchema#"
  xml:base="http://example.org/onto/">
  <owl:Class rdf:about="http://example.org/onto/class/aws_opensearchserverless_collection">
    <rdfs:label>aws_opensearchserverless_collection</rdfs:label>
    <rdfs:comment>Terraform resource for managing an AWS OpenSearch Serverless Collection.</rdfs:comment>
  </owl:Class>
  <owl:DatatypeProperty rdf:about="http://example.org/onto/prop/aws_opensearchserverless_collection_arn">
    <rdfs:label>arn</rdfs:label>
    <rdfs:domain rdf:resource="http://example.org/onto/class/aws_opensearchserverless_collection"/>
    <rdfs:range rdf:resource="http://www.w3.org/2001/XMLSchema#string"/>
  </owl:DatatypeProperty>
  <owl:DatatypeProperty rdf:about="http://example.org/onto/prop/aws_opensearchserverless_collection_collection_endpoint">
    <rdfs:label>collection_endpoint</rdfs:label>
    <rdfs:comment>Collection-specific endpoint used to submit index, search, and data upload requests to an OpenSearch Serverless collection.</rdfs:comment>
    <rdfs:domain rdf:resource="http://example.org/onto/class/aws_opensearchserverless_collection"/>
    <rdfs:range rdf:resource="http://www.w3.org/2001/XMLSchema#string"/>
  </owl:DatatypeProperty>
  <owl:DatatypeProperty rdf:about="http://example.org/onto/prop/aws_opensearchserverless_collection_dashboard_endpoint">
    <rdfs:label>dashboard_endpoint</rdfs:label>
    <rdfs:comment>Collection-specific endpoint used to access OpenSearch Dashboards.</rdfs:comment>
    <rdfs:domain rdf:resource="http://example.org/onto/class/aws_opensearchserverless_collection"/>
    <rdfs:range rdf:resource="http://www.w3.org/2001/XMLSchema#string"/>
  </owl:DatatypeProperty>
  <owl:DatatypeProperty rdf:about="http://example.org/onto/prop/aws_opensearchserverless_collection_description">
    <rdfs:label>description</rdfs:label>
    <rdfs:comment>Description of the collection.</rdfs:comment>
    <rdfs:domain rdf:resource="http://example.org/onto/class/aws_opensearchserverless_collection"/>
    <rdfs:range rdf:resource="http://www.w3.org/2001/XMLSchema#string"/>
  </owl:DatatypeProperty>
  <owl:DatatypeProperty rdf:about="http://example.org/onto/prop/aws_opensearchserverless_collection_id">
    <rdfs:label>id</rdfs:label>
    <rdfs:domain rdf:resource="http://example.org/onto/class/aws_opensearchserverless_collection"/>
    <rdfs:range rdf:resource="http://www.w3.org/2001/XMLSchema#string"/>
  </owl:DatatypeProperty>
  <owl:DatatypeProperty rdf:about="http://example.org/onto/prop/aws_opensearchserverless_collection_kms_key_arn">
    <rdfs:label>kms_key_arn</rdfs:label>
    <rdfs:comment>The ARN of the Amazon Web Services KMS key used to encrypt the collection.</rdfs:comment>
    <rdfs:domain rdf:resource="http://example.org/onto/class/aws_opensearchserverless_collection"/>
    <rdfs:range rdf:resource="http://www.w3.org/2001/XMLSchema#string"/>
  </owl:DatatypeProperty>
  <owl:DatatypeProperty rdf:about="http://example.org/onto/prop/aws_opensearchserverless_collection_name">
    <rdfs:label>name</rdfs:label>
    <rdfs:comment>Name of the collection.</rdfs:comment>
    <rdfs:domain rdf:resource="http://example.org/onto/class/aws_opensearchserverless_collection"/>
    <rdfs:range rdf:resource="http://www.w3.org/2001/XMLSchema#string"/>
  </owl:DatatypeProperty>
  <owl:DatatypeProperty rdf:about="http://example.org/onto/prop/aws_opensearchserverless_collection_region">
    <rdfs:label>region</rdfs:label>
    <rdfs:comment>Region where this resource will be [managed](https://docs.aws.amazon.com/general/latest/gr/rande.html#regional-endpoints). Defaults to the Region set in the [provider configuration](https://registry.terraform.io/providers/hashicorp/aws/latest/docs#aws-configuration-reference).</rdfs:comment>
    <rdfs:domain rdf:resource="http://example.org/onto/class/aws_opensearchserverless_collection"/>
    <rdfs:range rdf:resource="http://www.w3.org/2001/XMLSchema#string"/>
  </owl:DatatypeProperty>
  <owl:DatatypeProperty rdf:about="http://example.org/onto/prop/aws_opensearchserverless_collection_standby_replicas">
    <rdfs:label>standby_replicas</rdfs:label>
    <rdfs:comment>Indicates whether standby replicas should be used for a collection. One of `ENABLED` or `DISABLED`. Defaults to `ENABLED`.</rdfs:comment>
    <rdfs:domain rdf:resource="http://example.org/onto/class/aws_opensearchserverless_collection"/>
    <rdfs:range rdf:resource="http://www.w3.org/2001/XMLSchema#string"/>
  </owl:DatatypeProperty>
  <owl:DatatypeProperty rdf:about="http://example.org/onto/prop/aws_opensearchserverless_collection_tags">
    <rdfs:label>tags</rdfs:label>
    <rdfs:domain rdf:resource="http://example.org/onto/class/aws_opensearchserverless_collection"/>
    <rdfs:range rdf:resource="http://www.w3.org/2001/XMLSchema#string"/>
  </owl:DatatypeProperty>
  <owl:DatatypeProperty rdf:about="http://example.org/onto/prop/aws_opensearchserverless_collection_tags_all">
    <rdfs:label>tags_all</rdfs:label>
    <rdfs:domain rdf:resource="http://example.org/onto/class/aws_opensearchserverless_collection"/>
    <rdfs:range rdf:resource="http://www.w3.org/2001/XMLSchema#string"/>
  </owl:DatatypeProperty>
  <owl:DatatypeProperty rdf:about="http://example.org/onto/prop/aws_opensearchserverless_collection_type">
    <rdfs:label>type</rdfs:label>
    <rdfs:comment>Type of collection. One of `SEARCH`, `TIMESERIES`, or `VECTORSEARCH`. Defaults to `TIMESERIES`.</rdfs:comment>
    <rdfs:domain rdf:resource="http://example.org/onto/class/aws_opensearchserverless_collection"/>
    <rdfs:range rdf:resource="http://www.w3.org/2001/XMLSchema#string"/>
  </owl:DatatypeProperty>
  <owl:DatatypeProperty rdf:about="http://example.org/onto/prop/aws_opensearchserverless_collection_create">
    <rdfs:label>create</rdfs:label>
    <rdfs:comment>A string that can be [parsed as a duration](https://pkg.go.dev/time#ParseDuration) consisting of numbers and unit suffixes, such as "30s" or "2h45m". Valid time units are "s" (seconds), "m" (minutes), "h" (hours).</rdfs:comment>
    <rdfs:domain rdf:resource="http://example.org/onto/class/aws_opensearchserverless_collection"/>
    <rdfs:range rdf:resource="http://www.w3.org/2001/XMLSchema#string"/>
  </owl:DatatypeProperty>
  <owl:DatatypeProperty rdf:about="http://example.org/onto/prop/aws_opensearchserverless_collection_delete">
    <rdfs:label>delete</rdfs:label>
    <rdfs:comment>A string that can be [parsed as a duration](https://pkg.go.dev/time#ParseDuration) consisting of numbers and unit suffixes, such as "30s" or "2h45m". Valid time units are "s" (seconds), "m" (minutes), "h" (hours). Setting a timeout for a Delete operation is only applicable if changes are saved into state before the destroy operation occurs.</rdfs:comment>
    <rdfs:domain rdf:resource="http://example.org/onto/class/aws_opensearchserverless_collection"/>
    <rdfs:range rdf:resource="http://www.w3.org/2001/XMLSchema#string"/>
  </owl:DatatypeProperty>
</rdf:RDF>
