<?xml version="1.0" encoding="UTF-8"?>
<rdf:RDF
  xmlns:rdf="http://www.w3.org/1999/02/22-rdf-syntax-ns#"
  xmlns:rdfs="http://www.w3.org/2000/01/rdf-schema#"
  xmlns:owl="http://www.w3.org/2002/07/owl#"
  xmlns:xsd="http://www.w3.org/2001/XMLSchema#"
  xml:base="http://example.org/onto/">
  <owl:Class rdf:about="http://example.org/onto/class/aws_neptunegraph_graph">
    <rdfs:label>aws_neptunegraph_graph</rdfs:label>
    <rdfs:comment>The `aws_neptunegraph_graph` resource creates an Amazon Analytics Graph.</rdfs:comment>
  </owl:Class>
  <owl:DatatypeProperty rdf:about="http://example.org/onto/prop/aws_neptunegraph_graph_arn">
    <rdfs:label>arn</rdfs:label>
    <rdfs:domain rdf:resource="http://example.org/onto/class/aws_neptunegraph_graph"/>
    <rdfs:range rdf:resource="http://www.w3.org/2001/XMLSchema#string"/>
  </owl:DatatypeProperty>
  <owl:DatatypeProperty rdf:about="http://example.org/onto/prop/aws_neptunegraph_graph_deletion_protection">
    <rdfs:label>deletion_protection</rdfs:label>
    <rdfs:comment>A value that indicates whether the graph has deletion protection enabled. The graph can't be deleted when deletion protection is enabled.</rdfs:comment>
    <rdfs:domain rdf:resource="http://example.org/onto/class/aws_neptunegraph_graph"/>
    <rdfs:range rdf:resource="http://www.w3.org/2001/XMLSchema#string"/>
  </owl:DatatypeProperty>
  <owl:DatatypeProperty rdf:about="http://example.org/onto/prop/aws_neptunegraph_graph_endpoint">
    <rdfs:label>endpoint</rdfs:label>
    <rdfs:domain rdf:resource="http://example.org/onto/class/aws_neptunegraph_graph"/>
    <rdfs:range rdf:resource="http://www.w3.org/2001/XMLSchema#string"/>
  </owl:DatatypeProperty>
  <owl:DatatypeProperty rdf:about="http://example.org/onto/prop/aws_neptunegraph_graph_graph_name">
    <rdfs:label>graph_name</rdfs:label>
    <rdfs:comment>The graph name. For example: my-graph-1.
								The name must contain from 1 to 63 letters, numbers, or hyphens, 
								and its first character must be a letter. It cannot end with a hyphen or contain two consecutive hyphens.
								If you don't specify a graph name, a unique graph name is generated for you using the prefix graph-for, 
								followed by a combination of Stack Name and a UUID.</rdfs:comment>
    <rdfs:domain rdf:resource="http://example.org/onto/class/aws_neptunegraph_graph"/>
    <rdfs:range rdf:resource="http://www.w3.org/2001/XMLSchema#string"/>
  </owl:DatatypeProperty>
  <owl:DatatypeProperty rdf:about="http://example.org/onto/prop/aws_neptunegraph_graph_graph_name_prefix">
    <rdfs:label>graph_name_prefix</rdfs:label>
    <rdfs:comment>Allows user to specify name prefix and have remainder of name automatically generated.</rdfs:comment>
    <rdfs:domain rdf:resource="http://example.org/onto/class/aws_neptunegraph_graph"/>
    <rdfs:range rdf:resource="http://www.w3.org/2001/XMLSchema#string"/>
  </owl:DatatypeProperty>
  <owl:DatatypeProperty rdf:about="http://example.org/onto/prop/aws_neptunegraph_graph_id">
    <rdfs:label>id</rdfs:label>
    <rdfs:domain rdf:resource="http://example.org/onto/class/aws_neptunegraph_graph"/>
    <rdfs:range rdf:resource="http://www.w3.org/2001/XMLSchema#string"/>
  </owl:DatatypeProperty>
  <owl:DatatypeProperty rdf:about="http://example.org/onto/prop/aws_neptunegraph_graph_kms_key_identifier">
    <rdfs:label>kms_key_identifier</rdfs:label>
    <rdfs:comment>Specifies a KMS key to use to encrypt data in the new graph.  Value must be ARN of KMS Key.</rdfs:comment>
    <rdfs:domain rdf:resource="http://example.org/onto/class/aws_neptunegraph_graph"/>
    <rdfs:range rdf:resource="http://www.w3.org/2001/XMLSchema#string"/>
  </owl:DatatypeProperty>
  <owl:DatatypeProperty rdf:about="http://example.org/onto/prop/aws_neptunegraph_graph_provisioned_memory">
    <rdfs:label>provisioned_memory</rdfs:label>
    <rdfs:comment>The provisioned memory-optimized Neptune Capacity Units (m-NCUs) to use for the graph.</rdfs:comment>
    <rdfs:domain rdf:resource="http://example.org/onto/class/aws_neptunegraph_graph"/>
    <rdfs:range rdf:resource="http://www.w3.org/2001/XMLSchema#string"/>
  </owl:DatatypeProperty>
  <owl:DatatypeProperty rdf:about="http://example.org/onto/prop/aws_neptunegraph_graph_public_connectivity">
    <rdfs:label>public_connectivity</rdfs:label>
    <rdfs:comment>Specifies whether or not the graph can be reachable over the internet. 
								All access to graphs is IAM authenticated.
								When the graph is publicly available, its domain name system (DNS) endpoint resolves to 
								the public IP address from the internet. When the graph isn't publicly available, you need 
								to create a PrivateGraphEndpoint in a given VPC to ensure the DNS name resolves to a private 
								IP address that is reachable from the VPC.</rdfs:comment>
    <rdfs:domain rdf:resource="http://example.org/onto/class/aws_neptunegraph_graph"/>
    <rdfs:range rdf:resource="http://www.w3.org/2001/XMLSchema#string"/>
  </owl:DatatypeProperty>
  <owl:DatatypeProperty rdf:about="http://example.org/onto/prop/aws_neptunegraph_graph_region">
    <rdfs:label>region</rdfs:label>
    <rdfs:comment>Region where this resource will be [managed](https://docs.aws.amazon.com/general/latest/gr/rande.html#regional-endpoints). Defaults to the Region set in the [provider configuration](https://registry.terraform.io/providers/hashicorp/aws/latest/docs#aws-configuration-reference).</rdfs:comment>
    <rdfs:domain rdf:resource="http://example.org/onto/class/aws_neptunegraph_graph"/>
    <rdfs:range rdf:resource="http://www.w3.org/2001/XMLSchema#string"/>
  </owl:DatatypeProperty>
  <owl:DatatypeProperty rdf:about="http://example.org/onto/prop/aws_neptunegraph_graph_replica_count">
    <rdfs:label>replica_count</rdfs:label>
    <rdfs:comment>The number of replicas in other AZs.  Value must be between 0 and 2.</rdfs:comment>
    <rdfs:domain rdf:resource="http://example.org/onto/class/aws_neptunegraph_graph"/>
    <rdfs:range rdf:resource="http://www.w3.org/2001/XMLSchema#string"/>
  </owl:DatatypeProperty>
  <owl:DatatypeProperty rdf:about="http://example.org/onto/prop/aws_neptunegraph_graph_tags">
    <rdfs:label>tags</rdfs:label>
    <rdfs:domain rdf:resource="http://example.org/onto/class/aws_neptunegraph_graph"/>
    <rdfs:range rdf:resource="http://www.w3.org/2001/XMLSchema#string"/>
  </owl:DatatypeProperty>
  <owl:DatatypeProperty rdf:about="http://example.org/onto/prop/aws_neptunegraph_graph_tags_all">
    <rdfs:label>tags_all</rdfs:label>
    <rdfs:domain rdf:resource="http://example.org/onto/class/aws_neptunegraph_graph"/>
    <rdfs:range rdf:resource="http://www.w3.org/2001/XMLSchema#string"/>
  </owl:DatatypeProperty>
  <owl:DatatypeProperty rdf:about="http://example.org/onto/prop/aws_neptunegraph_graph_create">
    <rdfs:label>create</rdfs:label>
    <rdfs:comment>A string that can be [parsed as a duration](https://pkg.go.dev/time#ParseDuration) consisting of numbers and unit suffixes, such as "30s" or "2h45m". Valid time units are "s" (seconds), "m" (minutes), "h" (hours).</rdfs:comment>
    <rdfs:domain rdf:resource="http://example.org/onto/class/aws_neptunegraph_graph"/>
    <rdfs:range rdf:resource="http://www.w3.org/2001/XMLSchema#string"/>
  </owl:DatatypeProperty>
  <owl:DatatypeProperty rdf:about="http://example.org/onto/prop/aws_neptunegraph_graph_delete">
    <rdfs:label>delete</rdfs:label>
    <rdfs:comment>A string that can be [parsed as a duration](https://pkg.go.dev/time#ParseDuration) consisting of numbers and unit suffixes, such as "30s" or "2h45m". Valid time units are "s" (seconds), "m" (minutes), "h" (hours). Setting a timeout for a Delete operation is only applicable if changes are saved into state before the destroy operation occurs.</rdfs:comment>
    <rdfs:domain rdf:resource="http://example.org/onto/class/aws_neptunegraph_graph"/>
    <rdfs:range rdf:resource="http://www.w3.org/2001/XMLSchema#string"/>
  </owl:DatatypeProperty>
  <owl:DatatypeProperty rdf:about="http://example.org/onto/prop/aws_neptunegraph_graph_update">
    <rdfs:label>update</rdfs:label>
    <rdfs:comment>A string that can be [parsed as a duration](https://pkg.go.dev/time#ParseDuration) consisting of numbers and unit suffixes, such as "30s" or "2h45m". Valid time units are "s" (seconds), "m" (minutes), "h" (hours).</rdfs:comment>
    <rdfs:domain rdf:resource="http://example.org/onto/class/aws_neptunegraph_graph"/>
    <rdfs:range rdf:resource="http://www.w3.org/2001/XMLSchema#string"/>
  </owl:DatatypeProperty>
  <owl:DatatypeProperty rdf:about="http://example.org/onto/prop/aws_neptunegraph_graph_vector_search_dimension">
    <rdfs:label>vector_search_dimension</rdfs:label>
    <rdfs:comment>Specifies the number of dimensions for vector embeddings.  Value must be between 1 and 65,535.</rdfs:comment>
    <rdfs:domain rdf:resource="http://example.org/onto/class/aws_neptunegraph_graph"/>
    <rdfs:range rdf:resource="http://www.w3.org/2001/XMLSchema#string"/>
  </owl:DatatypeProperty>
</rdf:RDF>
