<?xml version="1.0" encoding="UTF-8"?>
<rdf:RDF
  xmlns:rdf="http://www.w3.org/1999/02/22-rdf-syntax-ns#"
  xmlns:rdfs="http://www.w3.org/2000/01/rdf-schema#"
  xmlns:owl="http://www.w3.org/2002/07/owl#"
  xmlns:xsd="http://www.w3.org/2001/XMLSchema#"
  xml:base="http://example.org/onto/">
  <owl:Class rdf:about="http://example.org/onto/class/aws_odb_cloud_autonomous_vm_cluster">
    <rdfs:label>aws_odb_cloud_autonomous_vm_cluster</rdfs:label>
    <rdfs:comment>Terraform resource managing cloud autonomous vm cluster in AWS for Oracle Database@AWS.</rdfs:comment>
  </owl:Class>
  <owl:DatatypeProperty rdf:about="http://example.org/onto/prop/aws_odb_cloud_autonomous_vm_cluster_arn">
    <rdfs:label>arn</rdfs:label>
    <rdfs:domain rdf:resource="http://example.org/onto/class/aws_odb_cloud_autonomous_vm_cluster"/>
    <rdfs:range rdf:resource="http://www.w3.org/2001/XMLSchema#string"/>
  </owl:DatatypeProperty>
  <owl:DatatypeProperty rdf:about="http://example.org/onto/prop/aws_odb_cloud_autonomous_vm_cluster_autonomous_data_storage_percentage">
    <rdfs:label>autonomous_data_storage_percentage</rdfs:label>
    <rdfs:comment>The progress of the current operation on the Autonomous VM cluster, as a percentage.</rdfs:comment>
    <rdfs:domain rdf:resource="http://example.org/onto/class/aws_odb_cloud_autonomous_vm_cluster"/>
    <rdfs:range rdf:resource="http://www.w3.org/2001/XMLSchema#string"/>
  </owl:DatatypeProperty>
  <owl:DatatypeProperty rdf:about="http://example.org/onto/prop/aws_odb_cloud_autonomous_vm_cluster_autonomous_data_storage_size_in_tbs">
    <rdfs:label>autonomous_data_storage_size_in_tbs</rdfs:label>
    <rdfs:comment>The data storage size allocated for Autonomous Databases in the Autonomous VM cluster, in TB. Changing this will force terraform to create new resource.</rdfs:comment>
    <rdfs:domain rdf:resource="http://example.org/onto/class/aws_odb_cloud_autonomous_vm_cluster"/>
    <rdfs:range rdf:resource="http://www.w3.org/2001/XMLSchema#string"/>
  </owl:DatatypeProperty>
  <owl:DatatypeProperty rdf:about="http://example.org/onto/prop/aws_odb_cloud_autonomous_vm_cluster_available_autonomous_data_storage_size_in_tbs">
    <rdfs:label>available_autonomous_data_storage_size_in_tbs</rdfs:label>
    <rdfs:comment>The available data storage space for Autonomous Databases in the Autonomous VM cluster, in TB.</rdfs:comment>
    <rdfs:domain rdf:resource="http://example.org/onto/class/aws_odb_cloud_autonomous_vm_cluster"/>
    <rdfs:range rdf:resource="http://www.w3.org/2001/XMLSchema#string"/>
  </owl:DatatypeProperty>
  <owl:DatatypeProperty rdf:about="http://example.org/onto/prop/aws_odb_cloud_autonomous_vm_cluster_available_container_databases">
    <rdfs:label>available_container_databases</rdfs:label>
    <rdfs:comment>The number of Autonomous CDBs that you can create with the currently available storage.</rdfs:comment>
    <rdfs:domain rdf:resource="http://example.org/onto/class/aws_odb_cloud_autonomous_vm_cluster"/>
    <rdfs:range rdf:resource="http://www.w3.org/2001/XMLSchema#string"/>
  </owl:DatatypeProperty>
  <owl:DatatypeProperty rdf:about="http://example.org/onto/prop/aws_odb_cloud_autonomous_vm_cluster_available_cpus">
    <rdfs:label>available_cpus</rdfs:label>
    <rdfs:comment>The number of CPU cores available for allocation to Autonomous Databases</rdfs:comment>
    <rdfs:domain rdf:resource="http://example.org/onto/class/aws_odb_cloud_autonomous_vm_cluster"/>
    <rdfs:range rdf:resource="http://www.w3.org/2001/XMLSchema#string"/>
  </owl:DatatypeProperty>
  <owl:DatatypeProperty rdf:about="http://example.org/onto/prop/aws_odb_cloud_autonomous_vm_cluster_cloud_exadata_infrastructure_id">
    <rdfs:label>cloud_exadata_infrastructure_id</rdfs:label>
    <rdfs:comment>Exadata infrastructure id. Changing this will force terraform to create new resource.</rdfs:comment>
    <rdfs:domain rdf:resource="http://example.org/onto/class/aws_odb_cloud_autonomous_vm_cluster"/>
    <rdfs:range rdf:resource="http://www.w3.org/2001/XMLSchema#string"/>
  </owl:DatatypeProperty>
  <owl:DatatypeProperty rdf:about="http://example.org/onto/prop/aws_odb_cloud_autonomous_vm_cluster_compute_model">
    <rdfs:label>compute_model</rdfs:label>
    <rdfs:comment>The compute model of the Autonomous VM cluster: ECPU or OCPU.</rdfs:comment>
    <rdfs:domain rdf:resource="http://example.org/onto/class/aws_odb_cloud_autonomous_vm_cluster"/>
    <rdfs:range rdf:resource="http://www.w3.org/2001/XMLSchema#string"/>
  </owl:DatatypeProperty>
  <owl:DatatypeProperty rdf:about="http://example.org/onto/prop/aws_odb_cloud_autonomous_vm_cluster_cpu_core_count">
    <rdfs:label>cpu_core_count</rdfs:label>
    <rdfs:comment>The total number of CPU cores in the Autonomous VM cluster.</rdfs:comment>
    <rdfs:domain rdf:resource="http://example.org/onto/class/aws_odb_cloud_autonomous_vm_cluster"/>
    <rdfs:range rdf:resource="http://www.w3.org/2001/XMLSchema#string"/>
  </owl:DatatypeProperty>
  <owl:DatatypeProperty rdf:about="http://example.org/onto/prop/aws_odb_cloud_autonomous_vm_cluster_cpu_core_count_per_node">
    <rdfs:label>cpu_core_count_per_node</rdfs:label>
    <rdfs:comment>The number of CPU cores enabled per node in the Autonomous VM cluster.</rdfs:comment>
    <rdfs:domain rdf:resource="http://example.org/onto/class/aws_odb_cloud_autonomous_vm_cluster"/>
    <rdfs:range rdf:resource="http://www.w3.org/2001/XMLSchema#string"/>
  </owl:DatatypeProperty>
  <owl:DatatypeProperty rdf:about="http://example.org/onto/prop/aws_odb_cloud_autonomous_vm_cluster_cpu_percentage">
    <rdfs:label>cpu_percentage</rdfs:label>
    <rdfs:comment>The percentage of total CPU cores currently in use in the Autonomous VM cluster.</rdfs:comment>
    <rdfs:domain rdf:resource="http://example.org/onto/class/aws_odb_cloud_autonomous_vm_cluster"/>
    <rdfs:range rdf:resource="http://www.w3.org/2001/XMLSchema#string"/>
  </owl:DatatypeProperty>
  <owl:DatatypeProperty rdf:about="http://example.org/onto/prop/aws_odb_cloud_autonomous_vm_cluster_created_at">
    <rdfs:label>created_at</rdfs:label>
    <rdfs:comment>The date and time when the Autonomous VM cluster was created.</rdfs:comment>
    <rdfs:domain rdf:resource="http://example.org/onto/class/aws_odb_cloud_autonomous_vm_cluster"/>
    <rdfs:range rdf:resource="http://www.w3.org/2001/XMLSchema#string"/>
  </owl:DatatypeProperty>
  <owl:DatatypeProperty rdf:about="http://example.org/onto/prop/aws_odb_cloud_autonomous_vm_cluster_data_storage_size_in_gbs">
    <rdfs:label>data_storage_size_in_gbs</rdfs:label>
    <rdfs:comment>The total data storage allocated to the Autonomous VM cluster, in GB.</rdfs:comment>
    <rdfs:domain rdf:resource="http://example.org/onto/class/aws_odb_cloud_autonomous_vm_cluster"/>
    <rdfs:range rdf:resource="http://www.w3.org/2001/XMLSchema#string"/>
  </owl:DatatypeProperty>
  <owl:DatatypeProperty rdf:about="http://example.org/onto/prop/aws_odb_cloud_autonomous_vm_cluster_data_storage_size_in_tbs">
    <rdfs:label>data_storage_size_in_tbs</rdfs:label>
    <rdfs:comment>The total data storage allocated to the Autonomous VM cluster, in TB.</rdfs:comment>
    <rdfs:domain rdf:resource="http://example.org/onto/class/aws_odb_cloud_autonomous_vm_cluster"/>
    <rdfs:range rdf:resource="http://www.w3.org/2001/XMLSchema#string"/>
  </owl:DatatypeProperty>
  <owl:DatatypeProperty rdf:about="http://example.org/onto/prop/aws_odb_cloud_autonomous_vm_cluster_db_servers">
    <rdfs:label>db_servers</rdfs:label>
    <rdfs:comment>The database servers in the Autonomous VM cluster. Changing this will force terraform to create new resource.</rdfs:comment>
    <rdfs:domain rdf:resource="http://example.org/onto/class/aws_odb_cloud_autonomous_vm_cluster"/>
    <rdfs:range rdf:resource="http://www.w3.org/2001/XMLSchema#string"/>
  </owl:DatatypeProperty>
  <owl:DatatypeProperty rdf:about="http://example.org/onto/prop/aws_odb_cloud_autonomous_vm_cluster_description">
    <rdfs:label>description</rdfs:label>
    <rdfs:comment>The description of the Autonomous VM cluster.</rdfs:comment>
    <rdfs:domain rdf:resource="http://example.org/onto/class/aws_odb_cloud_autonomous_vm_cluster"/>
    <rdfs:range rdf:resource="http://www.w3.org/2001/XMLSchema#string"/>
  </owl:DatatypeProperty>
  <owl:DatatypeProperty rdf:about="http://example.org/onto/prop/aws_odb_cloud_autonomous_vm_cluster_display_name">
    <rdfs:label>display_name</rdfs:label>
    <rdfs:comment>The display name of the Autonomous VM cluster. Changing this will force terraform to create new resource.</rdfs:comment>
    <rdfs:domain rdf:resource="http://example.org/onto/class/aws_odb_cloud_autonomous_vm_cluster"/>
    <rdfs:range rdf:resource="http://www.w3.org/2001/XMLSchema#string"/>
  </owl:DatatypeProperty>
  <owl:DatatypeProperty rdf:about="http://example.org/onto/prop/aws_odb_cloud_autonomous_vm_cluster_domain">
    <rdfs:label>domain</rdfs:label>
    <rdfs:comment>The domain name of the Autonomous VM cluster.</rdfs:comment>
    <rdfs:domain rdf:resource="http://example.org/onto/class/aws_odb_cloud_autonomous_vm_cluster"/>
    <rdfs:range rdf:resource="http://www.w3.org/2001/XMLSchema#string"/>
  </owl:DatatypeProperty>
  <owl:DatatypeProperty rdf:about="http://example.org/onto/prop/aws_odb_cloud_autonomous_vm_cluster_exadata_storage_in_tbs_lowest_scaled_value">
    <rdfs:label>exadata_storage_in_tbs_lowest_scaled_value</rdfs:label>
    <rdfs:comment>The minimum value to which you can scale down the Exadata storage, in TB.</rdfs:comment>
    <rdfs:domain rdf:resource="http://example.org/onto/class/aws_odb_cloud_autonomous_vm_cluster"/>
    <rdfs:range rdf:resource="http://www.w3.org/2001/XMLSchema#string"/>
  </owl:DatatypeProperty>
  <owl:DatatypeProperty rdf:about="http://example.org/onto/prop/aws_odb_cloud_autonomous_vm_cluster_hostname">
    <rdfs:label>hostname</rdfs:label>
    <rdfs:comment>The hostname of the Autonomous VM cluster.</rdfs:comment>
    <rdfs:domain rdf:resource="http://example.org/onto/class/aws_odb_cloud_autonomous_vm_cluster"/>
    <rdfs:range rdf:resource="http://www.w3.org/2001/XMLSchema#string"/>
  </owl:DatatypeProperty>
  <owl:DatatypeProperty rdf:about="http://example.org/onto/prop/aws_odb_cloud_autonomous_vm_cluster_id">
    <rdfs:label>id</rdfs:label>
    <rdfs:domain rdf:resource="http://example.org/onto/class/aws_odb_cloud_autonomous_vm_cluster"/>
    <rdfs:range rdf:resource="http://www.w3.org/2001/XMLSchema#string"/>
  </owl:DatatypeProperty>
  <owl:DatatypeProperty rdf:about="http://example.org/onto/prop/aws_odb_cloud_autonomous_vm_cluster_is_mtls_enabled_vm_cluster">
    <rdfs:label>is_mtls_enabled_vm_cluster</rdfs:label>
    <rdfs:comment>Indicates whether mutual TLS (mTLS) authentication is enabled for the Autonomous VM cluster. Changing this will force terraform to create new resource.</rdfs:comment>
    <rdfs:domain rdf:resource="http://example.org/onto/class/aws_odb_cloud_autonomous_vm_cluster"/>
    <rdfs:range rdf:resource="http://www.w3.org/2001/XMLSchema#string"/>
  </owl:DatatypeProperty>
  <owl:DatatypeProperty rdf:about="http://example.org/onto/prop/aws_odb_cloud_autonomous_vm_cluster_license_model">
    <rdfs:label>license_model</rdfs:label>
    <rdfs:comment>The license model for the Autonomous VM cluster. Valid values are LICENSE_INCLUDED or BRING_YOUR_OWN_LICENSE . Changing this will force terraform to create new resource.</rdfs:comment>
    <rdfs:domain rdf:resource="http://example.org/onto/class/aws_odb_cloud_autonomous_vm_cluster"/>
    <rdfs:range rdf:resource="http://www.w3.org/2001/XMLSchema#string"/>
  </owl:DatatypeProperty>
  <owl:DatatypeProperty rdf:about="http://example.org/onto/prop/aws_odb_cloud_autonomous_vm_cluster_max_acds_lowest_scaled_value">
    <rdfs:label>max_acds_lowest_scaled_value</rdfs:label>
    <rdfs:comment>The minimum value to which you can scale down the maximum number of Autonomous CDBs.</rdfs:comment>
    <rdfs:domain rdf:resource="http://example.org/onto/class/aws_odb_cloud_autonomous_vm_cluster"/>
    <rdfs:range rdf:resource="http://www.w3.org/2001/XMLSchema#string"/>
  </owl:DatatypeProperty>
  <owl:DatatypeProperty rdf:about="http://example.org/onto/prop/aws_odb_cloud_autonomous_vm_cluster_memory_per_oracle_compute_unit_in_gbs">
    <rdfs:label>memory_per_oracle_compute_unit_in_gbs</rdfs:label>
    <rdfs:comment>The amount of memory allocated per Oracle Compute Unit, in GB. Changing this will force terraform to create new resource.</rdfs:comment>
    <rdfs:domain rdf:resource="http://example.org/onto/class/aws_odb_cloud_autonomous_vm_cluster"/>
    <rdfs:range rdf:resource="http://www.w3.org/2001/XMLSchema#string"/>
  </owl:DatatypeProperty>
  <owl:DatatypeProperty rdf:about="http://example.org/onto/prop/aws_odb_cloud_autonomous_vm_cluster_memory_size_in_gbs">
    <rdfs:label>memory_size_in_gbs</rdfs:label>
    <rdfs:comment>The total amount of memory allocated to the Autonomous VM cluster, in gigabytes(GB).</rdfs:comment>
    <rdfs:domain rdf:resource="http://example.org/onto/class/aws_odb_cloud_autonomous_vm_cluster"/>
    <rdfs:range rdf:resource="http://www.w3.org/2001/XMLSchema#string"/>
  </owl:DatatypeProperty>
  <owl:DatatypeProperty rdf:about="http://example.org/onto/prop/aws_odb_cloud_autonomous_vm_cluster_node_count">
    <rdfs:label>node_count</rdfs:label>
    <rdfs:comment>The number of database server nodes in the Autonomous VM cluster.</rdfs:comment>
    <rdfs:domain rdf:resource="http://example.org/onto/class/aws_odb_cloud_autonomous_vm_cluster"/>
    <rdfs:range rdf:resource="http://www.w3.org/2001/XMLSchema#string"/>
  </owl:DatatypeProperty>
  <owl:DatatypeProperty rdf:about="http://example.org/onto/prop/aws_odb_cloud_autonomous_vm_cluster_non_provisionable_autonomous_container_databases">
    <rdfs:label>non_provisionable_autonomous_container_databases</rdfs:label>
    <rdfs:comment>The number of Autonomous CDBs that can't be provisioned because of resource constraints.</rdfs:comment>
    <rdfs:domain rdf:resource="http://example.org/onto/class/aws_odb_cloud_autonomous_vm_cluster"/>
    <rdfs:range rdf:resource="http://www.w3.org/2001/XMLSchema#string"/>
  </owl:DatatypeProperty>
  <owl:DatatypeProperty rdf:about="http://example.org/onto/prop/aws_odb_cloud_autonomous_vm_cluster_oci_resource_anchor_name">
    <rdfs:label>oci_resource_anchor_name</rdfs:label>
    <rdfs:comment>The name of the OCI resource anchor associated with this Autonomous VM cluster.</rdfs:comment>
    <rdfs:domain rdf:resource="http://example.org/onto/class/aws_odb_cloud_autonomous_vm_cluster"/>
    <rdfs:range rdf:resource="http://www.w3.org/2001/XMLSchema#string"/>
  </owl:DatatypeProperty>
  <owl:DatatypeProperty rdf:about="http://example.org/onto/prop/aws_odb_cloud_autonomous_vm_cluster_oci_url">
    <rdfs:label>oci_url</rdfs:label>
    <rdfs:comment>The URL for accessing the OCI console page for this Autonomous VM cluster.</rdfs:comment>
    <rdfs:domain rdf:resource="http://example.org/onto/class/aws_odb_cloud_autonomous_vm_cluster"/>
    <rdfs:range rdf:resource="http://www.w3.org/2001/XMLSchema#string"/>
  </owl:DatatypeProperty>
  <owl:DatatypeProperty rdf:about="http://example.org/onto/prop/aws_odb_cloud_autonomous_vm_cluster_ocid">
    <rdfs:label>ocid</rdfs:label>
    <rdfs:comment>The Oracle Cloud Identifier (OCID) of the Autonomous VM cluster.</rdfs:comment>
    <rdfs:domain rdf:resource="http://example.org/onto/class/aws_odb_cloud_autonomous_vm_cluster"/>
    <rdfs:range rdf:resource="http://www.w3.org/2001/XMLSchema#string"/>
  </owl:DatatypeProperty>
  <owl:DatatypeProperty rdf:about="http://example.org/onto/prop/aws_odb_cloud_autonomous_vm_cluster_odb_network_id">
    <rdfs:label>odb_network_id</rdfs:label>
    <rdfs:comment>The unique identifier of the ODB network associated with this Autonomous VM Cluster. Changing this will force terraform to create new resource.</rdfs:comment>
    <rdfs:domain rdf:resource="http://example.org/onto/class/aws_odb_cloud_autonomous_vm_cluster"/>
    <rdfs:range rdf:resource="http://www.w3.org/2001/XMLSchema#string"/>
  </owl:DatatypeProperty>
  <owl:DatatypeProperty rdf:about="http://example.org/onto/prop/aws_odb_cloud_autonomous_vm_cluster_odb_node_storage_size_in_gbs">
    <rdfs:label>odb_node_storage_size_in_gbs</rdfs:label>
    <rdfs:comment>The local node storage allocated to the Autonomous VM cluster, in gigabytes (GB)</rdfs:comment>
    <rdfs:domain rdf:resource="http://example.org/onto/class/aws_odb_cloud_autonomous_vm_cluster"/>
    <rdfs:range rdf:resource="http://www.w3.org/2001/XMLSchema#string"/>
  </owl:DatatypeProperty>
  <owl:DatatypeProperty rdf:about="http://example.org/onto/prop/aws_odb_cloud_autonomous_vm_cluster_percent_progress">
    <rdfs:label>percent_progress</rdfs:label>
    <rdfs:comment>The progress of the current operation on the Autonomous VM cluster, as a percentage.</rdfs:comment>
    <rdfs:domain rdf:resource="http://example.org/onto/class/aws_odb_cloud_autonomous_vm_cluster"/>
    <rdfs:range rdf:resource="http://www.w3.org/2001/XMLSchema#string"/>
  </owl:DatatypeProperty>
  <owl:DatatypeProperty rdf:about="http://example.org/onto/prop/aws_odb_cloud_autonomous_vm_cluster_provisionable_autonomous_container_databases">
    <rdfs:label>provisionable_autonomous_container_databases</rdfs:label>
    <rdfs:comment>The number of Autonomous CDBs that can be provisioned in the Autonomous VM cluster.</rdfs:comment>
    <rdfs:domain rdf:resource="http://example.org/onto/class/aws_odb_cloud_autonomous_vm_cluster"/>
    <rdfs:range rdf:resource="http://www.w3.org/2001/XMLSchema#string"/>
  </owl:DatatypeProperty>
  <owl:DatatypeProperty rdf:about="http://example.org/onto/prop/aws_odb_cloud_autonomous_vm_cluster_provisioned_autonomous_container_databases">
    <rdfs:label>provisioned_autonomous_container_databases</rdfs:label>
    <rdfs:comment>The number of Autonomous CDBs currently provisioned in the Autonomous VM cluster.</rdfs:comment>
    <rdfs:domain rdf:resource="http://example.org/onto/class/aws_odb_cloud_autonomous_vm_cluster"/>
    <rdfs:range rdf:resource="http://www.w3.org/2001/XMLSchema#string"/>
  </owl:DatatypeProperty>
  <owl:DatatypeProperty rdf:about="http://example.org/onto/prop/aws_odb_cloud_autonomous_vm_cluster_provisioned_cpus">
    <rdfs:label>provisioned_cpus</rdfs:label>
    <rdfs:comment>The number of CPUs provisioned in the Autonomous VM cluster.</rdfs:comment>
    <rdfs:domain rdf:resource="http://example.org/onto/class/aws_odb_cloud_autonomous_vm_cluster"/>
    <rdfs:range rdf:resource="http://www.w3.org/2001/XMLSchema#string"/>
  </owl:DatatypeProperty>
  <owl:DatatypeProperty rdf:about="http://example.org/onto/prop/aws_odb_cloud_autonomous_vm_cluster_reclaimable_cpus">
    <rdfs:label>reclaimable_cpus</rdfs:label>
    <rdfs:comment>The number of CPU cores that can be reclaimed from terminated or scaled-down Autonomous Databases.</rdfs:comment>
    <rdfs:domain rdf:resource="http://example.org/onto/class/aws_odb_cloud_autonomous_vm_cluster"/>
    <rdfs:range rdf:resource="http://www.w3.org/2001/XMLSchema#string"/>
  </owl:DatatypeProperty>
  <owl:DatatypeProperty rdf:about="http://example.org/onto/prop/aws_odb_cloud_autonomous_vm_cluster_region">
    <rdfs:label>region</rdfs:label>
    <rdfs:comment>Region where this resource will be [managed](https://docs.aws.amazon.com/general/latest/gr/rande.html#regional-endpoints). Defaults to the Region set in the [provider configuration](https://registry.terraform.io/providers/hashicorp/aws/latest/docs#aws-configuration-reference).</rdfs:comment>
    <rdfs:domain rdf:resource="http://example.org/onto/class/aws_odb_cloud_autonomous_vm_cluster"/>
    <rdfs:range rdf:resource="http://www.w3.org/2001/XMLSchema#string"/>
  </owl:DatatypeProperty>
  <owl:DatatypeProperty rdf:about="http://example.org/onto/prop/aws_odb_cloud_autonomous_vm_cluster_reserved_cpus">
    <rdfs:label>reserved_cpus</rdfs:label>
    <rdfs:comment>The number of CPU cores reserved for system operations and redundancy.</rdfs:comment>
    <rdfs:domain rdf:resource="http://example.org/onto/class/aws_odb_cloud_autonomous_vm_cluster"/>
    <rdfs:range rdf:resource="http://www.w3.org/2001/XMLSchema#string"/>
  </owl:DatatypeProperty>
  <owl:DatatypeProperty rdf:about="http://example.org/onto/prop/aws_odb_cloud_autonomous_vm_cluster_scan_listener_port_non_tls">
    <rdfs:label>scan_listener_port_non_tls</rdfs:label>
    <rdfs:comment>The SCAN listener port for non-TLS (TCP) protocol. The default is 1521. Changing this will force terraform to create new resource.</rdfs:comment>
    <rdfs:domain rdf:resource="http://example.org/onto/class/aws_odb_cloud_autonomous_vm_cluster"/>
    <rdfs:range rdf:resource="http://www.w3.org/2001/XMLSchema#string"/>
  </owl:DatatypeProperty>
  <owl:DatatypeProperty rdf:about="http://example.org/onto/prop/aws_odb_cloud_autonomous_vm_cluster_scan_listener_port_tls">
    <rdfs:label>scan_listener_port_tls</rdfs:label>
    <rdfs:comment>The SCAN listener port for TLS (TCP) protocol. The default is 2484. Changing this will force terraform to create new resource.</rdfs:comment>
    <rdfs:domain rdf:resource="http://example.org/onto/class/aws_odb_cloud_autonomous_vm_cluster"/>
    <rdfs:range rdf:resource="http://www.w3.org/2001/XMLSchema#string"/>
  </owl:DatatypeProperty>
  <owl:DatatypeProperty rdf:about="http://example.org/onto/prop/aws_odb_cloud_autonomous_vm_cluster_shape">
    <rdfs:label>shape</rdfs:label>
    <rdfs:comment>The shape of the Exadata infrastructure for the Autonomous VM cluster.</rdfs:comment>
    <rdfs:domain rdf:resource="http://example.org/onto/class/aws_odb_cloud_autonomous_vm_cluster"/>
    <rdfs:range rdf:resource="http://www.w3.org/2001/XMLSchema#string"/>
  </owl:DatatypeProperty>
  <owl:DatatypeProperty rdf:about="http://example.org/onto/prop/aws_odb_cloud_autonomous_vm_cluster_status">
    <rdfs:label>status</rdfs:label>
    <rdfs:comment>The status of the Autonomous VM cluster. Possible values include CREATING, AVAILABLE , UPDATING , DELETING , DELETED , FAILED</rdfs:comment>
    <rdfs:domain rdf:resource="http://example.org/onto/class/aws_odb_cloud_autonomous_vm_cluster"/>
    <rdfs:range rdf:resource="http://www.w3.org/2001/XMLSchema#string"/>
  </owl:DatatypeProperty>
  <owl:DatatypeProperty rdf:about="http://example.org/onto/prop/aws_odb_cloud_autonomous_vm_cluster_status_reason">
    <rdfs:label>status_reason</rdfs:label>
    <rdfs:comment>Additional information about the current status of the Autonomous VM cluster.</rdfs:comment>
    <rdfs:domain rdf:resource="http://example.org/onto/class/aws_odb_cloud_autonomous_vm_cluster"/>
    <rdfs:range rdf:resource="http://www.w3.org/2001/XMLSchema#string"/>
  </owl:DatatypeProperty>
  <owl:DatatypeProperty rdf:about="http://example.org/onto/prop/aws_odb_cloud_autonomous_vm_cluster_tags">
    <rdfs:label>tags</rdfs:label>
    <rdfs:domain rdf:resource="http://example.org/onto/class/aws_odb_cloud_autonomous_vm_cluster"/>
    <rdfs:range rdf:resource="http://www.w3.org/2001/XMLSchema#string"/>
  </owl:DatatypeProperty>
  <owl:DatatypeProperty rdf:about="http://example.org/onto/prop/aws_odb_cloud_autonomous_vm_cluster_tags_all">
    <rdfs:label>tags_all</rdfs:label>
    <rdfs:domain rdf:resource="http://example.org/onto/class/aws_odb_cloud_autonomous_vm_cluster"/>
    <rdfs:range rdf:resource="http://www.w3.org/2001/XMLSchema#string"/>
  </owl:DatatypeProperty>
  <owl:DatatypeProperty rdf:about="http://example.org/onto/prop/aws_odb_cloud_autonomous_vm_cluster_time_database_ssl_certificate_expires">
    <rdfs:label>time_database_ssl_certificate_expires</rdfs:label>
    <rdfs:comment>The expiration date and time of the database SSL certificate.</rdfs:comment>
    <rdfs:domain rdf:resource="http://example.org/onto/class/aws_odb_cloud_autonomous_vm_cluster"/>
    <rdfs:range rdf:resource="http://www.w3.org/2001/XMLSchema#string"/>
  </owl:DatatypeProperty>
  <owl:DatatypeProperty rdf:about="http://example.org/onto/prop/aws_odb_cloud_autonomous_vm_cluster_time_ords_certificate_expires">
    <rdfs:label>time_ords_certificate_expires</rdfs:label>
    <rdfs:domain rdf:resource="http://example.org/onto/class/aws_odb_cloud_autonomous_vm_cluster"/>
    <rdfs:range rdf:resource="http://www.w3.org/2001/XMLSchema#string"/>
  </owl:DatatypeProperty>
  <owl:DatatypeProperty rdf:about="http://example.org/onto/prop/aws_odb_cloud_autonomous_vm_cluster_time_zone">
    <rdfs:label>time_zone</rdfs:label>
    <rdfs:comment>The time zone of the Autonomous VM cluster. Changing this will force terraform to create new resource.</rdfs:comment>
    <rdfs:domain rdf:resource="http://example.org/onto/class/aws_odb_cloud_autonomous_vm_cluster"/>
    <rdfs:range rdf:resource="http://www.w3.org/2001/XMLSchema#string"/>
  </owl:DatatypeProperty>
  <owl:DatatypeProperty rdf:about="http://example.org/onto/prop/aws_odb_cloud_autonomous_vm_cluster_total_container_databases">
    <rdfs:label>total_container_databases</rdfs:label>
    <rdfs:comment>The total number of Autonomous Container Databases that can be created with the allocated local storage. Changing this will force terraform to create new resource.</rdfs:comment>
    <rdfs:domain rdf:resource="http://example.org/onto/class/aws_odb_cloud_autonomous_vm_cluster"/>
    <rdfs:range rdf:resource="http://www.w3.org/2001/XMLSchema#string"/>
  </owl:DatatypeProperty>
  <owl:DatatypeProperty rdf:about="http://example.org/onto/prop/aws_odb_cloud_autonomous_vm_cluster_days_of_week">
    <rdfs:label>days_of_week</rdfs:label>
    <rdfs:comment>The days of the week when maintenance can be performed.</rdfs:comment>
    <rdfs:domain rdf:resource="http://example.org/onto/class/aws_odb_cloud_autonomous_vm_cluster"/>
    <rdfs:range rdf:resource="http://www.w3.org/2001/XMLSchema#string"/>
  </owl:DatatypeProperty>
  <owl:DatatypeProperty rdf:about="http://example.org/onto/prop/aws_odb_cloud_autonomous_vm_cluster_hours_of_day">
    <rdfs:label>hours_of_day</rdfs:label>
    <rdfs:comment>The hours of the day when maintenance can be performed.</rdfs:comment>
    <rdfs:domain rdf:resource="http://example.org/onto/class/aws_odb_cloud_autonomous_vm_cluster"/>
    <rdfs:range rdf:resource="http://www.w3.org/2001/XMLSchema#string"/>
  </owl:DatatypeProperty>
  <owl:DatatypeProperty rdf:about="http://example.org/onto/prop/aws_odb_cloud_autonomous_vm_cluster_lead_time_in_weeks">
    <rdfs:label>lead_time_in_weeks</rdfs:label>
    <rdfs:comment>The lead time in weeks before the maintenance window.</rdfs:comment>
    <rdfs:domain rdf:resource="http://example.org/onto/class/aws_odb_cloud_autonomous_vm_cluster"/>
    <rdfs:range rdf:resource="http://www.w3.org/2001/XMLSchema#string"/>
  </owl:DatatypeProperty>
  <owl:DatatypeProperty rdf:about="http://example.org/onto/prop/aws_odb_cloud_autonomous_vm_cluster_months">
    <rdfs:label>months</rdfs:label>
    <rdfs:comment>The months when maintenance can be performed.</rdfs:comment>
    <rdfs:domain rdf:resource="http://example.org/onto/class/aws_odb_cloud_autonomous_vm_cluster"/>
    <rdfs:range rdf:resource="http://www.w3.org/2001/XMLSchema#string"/>
  </owl:DatatypeProperty>
  <owl:DatatypeProperty rdf:about="http://example.org/onto/prop/aws_odb_cloud_autonomous_vm_cluster_preference">
    <rdfs:label>preference</rdfs:label>
    <rdfs:comment>The preference for the maintenance window scheduling.</rdfs:comment>
    <rdfs:domain rdf:resource="http://example.org/onto/class/aws_odb_cloud_autonomous_vm_cluster"/>
    <rdfs:range rdf:resource="http://www.w3.org/2001/XMLSchema#string"/>
  </owl:DatatypeProperty>
  <owl:DatatypeProperty rdf:about="http://example.org/onto/prop/aws_odb_cloud_autonomous_vm_cluster_weeks_of_month">
    <rdfs:label>weeks_of_month</rdfs:label>
    <rdfs:comment>Indicates whether to skip release updates during maintenance.</rdfs:comment>
    <rdfs:domain rdf:resource="http://example.org/onto/class/aws_odb_cloud_autonomous_vm_cluster"/>
    <rdfs:range rdf:resource="http://www.w3.org/2001/XMLSchema#string"/>
  </owl:DatatypeProperty>
  <owl:DatatypeProperty rdf:about="http://example.org/onto/prop/aws_odb_cloud_autonomous_vm_cluster_create">
    <rdfs:label>create</rdfs:label>
    <rdfs:comment>A string that can be [parsed as a duration](https://pkg.go.dev/time#ParseDuration) consisting of numbers and unit suffixes, such as "30s" or "2h45m". Valid time units are "s" (seconds), "m" (minutes), "h" (hours).</rdfs:comment>
    <rdfs:domain rdf:resource="http://example.org/onto/class/aws_odb_cloud_autonomous_vm_cluster"/>
    <rdfs:range rdf:resource="http://www.w3.org/2001/XMLSchema#string"/>
  </owl:DatatypeProperty>
  <owl:DatatypeProperty rdf:about="http://example.org/onto/prop/aws_odb_cloud_autonomous_vm_cluster_delete">
    <rdfs:label>delete</rdfs:label>
    <rdfs:comment>A string that can be [parsed as a duration](https://pkg.go.dev/time#ParseDuration) consisting of numbers and unit suffixes, such as "30s" or "2h45m". Valid time units are "s" (seconds), "m" (minutes), "h" (hours). Setting a timeout for a Delete operation is only applicable if changes are saved into state before the destroy operation occurs.</rdfs:comment>
    <rdfs:domain rdf:resource="http://example.org/onto/class/aws_odb_cloud_autonomous_vm_cluster"/>
    <rdfs:range rdf:resource="http://www.w3.org/2001/XMLSchema#string"/>
  </owl:DatatypeProperty>
  <owl:DatatypeProperty rdf:about="http://example.org/onto/prop/aws_odb_cloud_autonomous_vm_cluster_update">
    <rdfs:label>update</rdfs:label>
    <rdfs:comment>A string that can be [parsed as a duration](https://pkg.go.dev/time#ParseDuration) consisting of numbers and unit suffixes, such as "30s" or "2h45m". Valid time units are "s" (seconds), "m" (minutes), "h" (hours).</rdfs:comment>
    <rdfs:domain rdf:resource="http://example.org/onto/class/aws_odb_cloud_autonomous_vm_cluster"/>
    <rdfs:range rdf:resource="http://www.w3.org/2001/XMLSchema#string"/>
  </owl:DatatypeProperty>
</rdf:RDF>
