<?xml version="1.0" encoding="UTF-8"?>
<rdf:RDF
  xmlns:rdf="http://www.w3.org/1999/02/22-rdf-syntax-ns#"
  xmlns:rdfs="http://www.w3.org/2000/01/rdf-schema#"
  xmlns:owl="http://www.w3.org/2002/07/owl#"
  xmlns:xsd="http://www.w3.org/2001/XMLSchema#"
  xml:base="http://example.org/onto/">
  <owl:Class rdf:about="http://example.org/onto/class/aws_rekognition_stream_processor">
    <rdfs:label>aws_rekognition_stream_processor</rdfs:label>
    <rdfs:comment>Terraform resource for managing an AWS Rekognition Stream Processor.</rdfs:comment>
  </owl:Class>
  <owl:DatatypeProperty rdf:about="http://example.org/onto/prop/aws_rekognition_stream_processor_arn">
    <rdfs:label>arn</rdfs:label>
    <rdfs:domain rdf:resource="http://example.org/onto/class/aws_rekognition_stream_processor"/>
    <rdfs:range rdf:resource="http://www.w3.org/2001/XMLSchema#string"/>
  </owl:DatatypeProperty>
  <owl:DatatypeProperty rdf:about="http://example.org/onto/prop/aws_rekognition_stream_processor_kms_key_id">
    <rdfs:label>kms_key_id</rdfs:label>
    <rdfs:comment>The identifier for your AWS Key Management Service key (AWS KMS key). You can supply the Amazon Resource Name (ARN) of your KMS key, the ID of your KMS key, an alias for your KMS key, or an alias ARN.</rdfs:comment>
    <rdfs:domain rdf:resource="http://example.org/onto/class/aws_rekognition_stream_processor"/>
    <rdfs:range rdf:resource="http://www.w3.org/2001/XMLSchema#string"/>
  </owl:DatatypeProperty>
  <owl:DatatypeProperty rdf:about="http://example.org/onto/prop/aws_rekognition_stream_processor_name">
    <rdfs:label>name</rdfs:label>
    <rdfs:comment>An identifier you assign to the stream processor.</rdfs:comment>
    <rdfs:domain rdf:resource="http://example.org/onto/class/aws_rekognition_stream_processor"/>
    <rdfs:range rdf:resource="http://www.w3.org/2001/XMLSchema#string"/>
  </owl:DatatypeProperty>
  <owl:DatatypeProperty rdf:about="http://example.org/onto/prop/aws_rekognition_stream_processor_region">
    <rdfs:label>region</rdfs:label>
    <rdfs:comment>Region where this resource will be [managed](https://docs.aws.amazon.com/general/latest/gr/rande.html#regional-endpoints). Defaults to the Region set in the [provider configuration](https://registry.terraform.io/providers/hashicorp/aws/latest/docs#aws-configuration-reference).</rdfs:comment>
    <rdfs:domain rdf:resource="http://example.org/onto/class/aws_rekognition_stream_processor"/>
    <rdfs:range rdf:resource="http://www.w3.org/2001/XMLSchema#string"/>
  </owl:DatatypeProperty>
  <owl:DatatypeProperty rdf:about="http://example.org/onto/prop/aws_rekognition_stream_processor_role_arn">
    <rdfs:label>role_arn</rdfs:label>
    <rdfs:comment>The Amazon Resource Number (ARN) of the IAM role that allows access to the stream processor.</rdfs:comment>
    <rdfs:domain rdf:resource="http://example.org/onto/class/aws_rekognition_stream_processor"/>
    <rdfs:range rdf:resource="http://www.w3.org/2001/XMLSchema#string"/>
  </owl:DatatypeProperty>
  <owl:DatatypeProperty rdf:about="http://example.org/onto/prop/aws_rekognition_stream_processor_stream_processor_arn">
    <rdfs:label>stream_processor_arn</rdfs:label>
    <rdfs:domain rdf:resource="http://example.org/onto/class/aws_rekognition_stream_processor"/>
    <rdfs:range rdf:resource="http://www.w3.org/2001/XMLSchema#string"/>
  </owl:DatatypeProperty>
  <owl:DatatypeProperty rdf:about="http://example.org/onto/prop/aws_rekognition_stream_processor_tags">
    <rdfs:label>tags</rdfs:label>
    <rdfs:domain rdf:resource="http://example.org/onto/class/aws_rekognition_stream_processor"/>
    <rdfs:range rdf:resource="http://www.w3.org/2001/XMLSchema#string"/>
  </owl:DatatypeProperty>
  <owl:DatatypeProperty rdf:about="http://example.org/onto/prop/aws_rekognition_stream_processor_tags_all">
    <rdfs:label>tags_all</rdfs:label>
    <rdfs:domain rdf:resource="http://example.org/onto/class/aws_rekognition_stream_processor"/>
    <rdfs:range rdf:resource="http://www.w3.org/2001/XMLSchema#string"/>
  </owl:DatatypeProperty>
  <owl:DatatypeProperty rdf:about="http://example.org/onto/prop/aws_rekognition_stream_processor_opt_in">
    <rdfs:label>opt_in</rdfs:label>
    <rdfs:comment>Do you want to share data with Rekognition to improve model performance.</rdfs:comment>
    <rdfs:domain rdf:resource="http://example.org/onto/class/aws_rekognition_stream_processor"/>
    <rdfs:range rdf:resource="http://www.w3.org/2001/XMLSchema#string"/>
  </owl:DatatypeProperty>
  <owl:DatatypeProperty rdf:about="http://example.org/onto/prop/aws_rekognition_stream_processor_arn">
    <rdfs:label>arn</rdfs:label>
    <rdfs:comment>ARN of the Kinesis video stream stream that streams the source video.</rdfs:comment>
    <rdfs:domain rdf:resource="http://example.org/onto/class/aws_rekognition_stream_processor"/>
    <rdfs:range rdf:resource="http://www.w3.org/2001/XMLSchema#string"/>
  </owl:DatatypeProperty>
  <owl:DatatypeProperty rdf:about="http://example.org/onto/prop/aws_rekognition_stream_processor_sns_topic_arn">
    <rdfs:label>sns_topic_arn</rdfs:label>
    <rdfs:comment>The Amazon Resource Number (ARN) of the Amazon Amazon Simple Notification Service topic to which Amazon Rekognition posts the completion status.</rdfs:comment>
    <rdfs:domain rdf:resource="http://example.org/onto/class/aws_rekognition_stream_processor"/>
    <rdfs:range rdf:resource="http://www.w3.org/2001/XMLSchema#string"/>
  </owl:DatatypeProperty>
  <owl:DatatypeProperty rdf:about="http://example.org/onto/prop/aws_rekognition_stream_processor_arn">
    <rdfs:label>arn</rdfs:label>
    <rdfs:comment>ARN of the output Amazon Kinesis Data Streams stream.</rdfs:comment>
    <rdfs:domain rdf:resource="http://example.org/onto/class/aws_rekognition_stream_processor"/>
    <rdfs:range rdf:resource="http://www.w3.org/2001/XMLSchema#string"/>
  </owl:DatatypeProperty>
  <owl:DatatypeProperty rdf:about="http://example.org/onto/prop/aws_rekognition_stream_processor_bucket">
    <rdfs:label>bucket</rdfs:label>
    <rdfs:comment>The name of the Amazon S3 bucket you want to associate with the streaming video project.</rdfs:comment>
    <rdfs:domain rdf:resource="http://example.org/onto/class/aws_rekognition_stream_processor"/>
    <rdfs:range rdf:resource="http://www.w3.org/2001/XMLSchema#string"/>
  </owl:DatatypeProperty>
  <owl:DatatypeProperty rdf:about="http://example.org/onto/prop/aws_rekognition_stream_processor_key_prefix">
    <rdfs:label>key_prefix</rdfs:label>
    <rdfs:comment>The prefix value of the location within the bucket that you want the information to be published to.</rdfs:comment>
    <rdfs:domain rdf:resource="http://example.org/onto/class/aws_rekognition_stream_processor"/>
    <rdfs:range rdf:resource="http://www.w3.org/2001/XMLSchema#string"/>
  </owl:DatatypeProperty>
  <owl:DatatypeProperty rdf:about="http://example.org/onto/prop/aws_rekognition_stream_processor_height">
    <rdfs:label>height</rdfs:label>
    <rdfs:comment>Height of the bounding box as a ratio of the overall image height.</rdfs:comment>
    <rdfs:domain rdf:resource="http://example.org/onto/class/aws_rekognition_stream_processor"/>
    <rdfs:range rdf:resource="http://www.w3.org/2001/XMLSchema#string"/>
  </owl:DatatypeProperty>
  <owl:DatatypeProperty rdf:about="http://example.org/onto/prop/aws_rekognition_stream_processor_left">
    <rdfs:label>left</rdfs:label>
    <rdfs:comment>Left coordinate of the bounding box as a ratio of overall image width.</rdfs:comment>
    <rdfs:domain rdf:resource="http://example.org/onto/class/aws_rekognition_stream_processor"/>
    <rdfs:range rdf:resource="http://www.w3.org/2001/XMLSchema#string"/>
  </owl:DatatypeProperty>
  <owl:DatatypeProperty rdf:about="http://example.org/onto/prop/aws_rekognition_stream_processor_top">
    <rdfs:label>top</rdfs:label>
    <rdfs:comment>Top coordinate of the bounding box as a ratio of overall image height.</rdfs:comment>
    <rdfs:domain rdf:resource="http://example.org/onto/class/aws_rekognition_stream_processor"/>
    <rdfs:range rdf:resource="http://www.w3.org/2001/XMLSchema#string"/>
  </owl:DatatypeProperty>
  <owl:DatatypeProperty rdf:about="http://example.org/onto/prop/aws_rekognition_stream_processor_width">
    <rdfs:label>width</rdfs:label>
    <rdfs:comment>Width of the bounding box as a ratio of the overall image width.</rdfs:comment>
    <rdfs:domain rdf:resource="http://example.org/onto/class/aws_rekognition_stream_processor"/>
    <rdfs:range rdf:resource="http://www.w3.org/2001/XMLSchema#string"/>
  </owl:DatatypeProperty>
  <owl:DatatypeProperty rdf:about="http://example.org/onto/prop/aws_rekognition_stream_processor_x">
    <rdfs:label>x</rdfs:label>
    <rdfs:comment>The value of the X coordinate for a point on a Polygon.</rdfs:comment>
    <rdfs:domain rdf:resource="http://example.org/onto/class/aws_rekognition_stream_processor"/>
    <rdfs:range rdf:resource="http://www.w3.org/2001/XMLSchema#string"/>
  </owl:DatatypeProperty>
  <owl:DatatypeProperty rdf:about="http://example.org/onto/prop/aws_rekognition_stream_processor_y">
    <rdfs:label>y</rdfs:label>
    <rdfs:comment>The value of the Y coordinate for a point on a Polygon.</rdfs:comment>
    <rdfs:domain rdf:resource="http://example.org/onto/class/aws_rekognition_stream_processor"/>
    <rdfs:range rdf:resource="http://www.w3.org/2001/XMLSchema#string"/>
  </owl:DatatypeProperty>
  <owl:DatatypeProperty rdf:about="http://example.org/onto/prop/aws_rekognition_stream_processor_labels">
    <rdfs:label>labels</rdfs:label>
    <rdfs:comment>Specifies what you want to detect in the video, such as people, packages, or pets.</rdfs:comment>
    <rdfs:domain rdf:resource="http://example.org/onto/class/aws_rekognition_stream_processor"/>
    <rdfs:range rdf:resource="http://www.w3.org/2001/XMLSchema#string"/>
  </owl:DatatypeProperty>
  <owl:DatatypeProperty rdf:about="http://example.org/onto/prop/aws_rekognition_stream_processor_min_confidence">
    <rdfs:label>min_confidence</rdfs:label>
    <rdfs:comment>The minimum confidence required to label an object in the video.</rdfs:comment>
    <rdfs:domain rdf:resource="http://example.org/onto/class/aws_rekognition_stream_processor"/>
    <rdfs:range rdf:resource="http://www.w3.org/2001/XMLSchema#string"/>
  </owl:DatatypeProperty>
  <owl:DatatypeProperty rdf:about="http://example.org/onto/prop/aws_rekognition_stream_processor_collection_id">
    <rdfs:label>collection_id</rdfs:label>
    <rdfs:comment>The ID of a collection that contains faces that you want to search for.</rdfs:comment>
    <rdfs:domain rdf:resource="http://example.org/onto/class/aws_rekognition_stream_processor"/>
    <rdfs:range rdf:resource="http://www.w3.org/2001/XMLSchema#string"/>
  </owl:DatatypeProperty>
  <owl:DatatypeProperty rdf:about="http://example.org/onto/prop/aws_rekognition_stream_processor_face_match_threshold">
    <rdfs:label>face_match_threshold</rdfs:label>
    <rdfs:comment>Minimum face match confidence score that must be met to return a result for a recognized face.</rdfs:comment>
    <rdfs:domain rdf:resource="http://example.org/onto/class/aws_rekognition_stream_processor"/>
    <rdfs:range rdf:resource="http://www.w3.org/2001/XMLSchema#string"/>
  </owl:DatatypeProperty>
  <owl:DatatypeProperty rdf:about="http://example.org/onto/prop/aws_rekognition_stream_processor_create">
    <rdfs:label>create</rdfs:label>
    <rdfs:comment>A string that can be [parsed as a duration](https://pkg.go.dev/time#ParseDuration) consisting of numbers and unit suffixes, such as "30s" or "2h45m". Valid time units are "s" (seconds), "m" (minutes), "h" (hours).</rdfs:comment>
    <rdfs:domain rdf:resource="http://example.org/onto/class/aws_rekognition_stream_processor"/>
    <rdfs:range rdf:resource="http://www.w3.org/2001/XMLSchema#string"/>
  </owl:DatatypeProperty>
  <owl:DatatypeProperty rdf:about="http://example.org/onto/prop/aws_rekognition_stream_processor_delete">
    <rdfs:label>delete</rdfs:label>
    <rdfs:comment>A string that can be [parsed as a duration](https://pkg.go.dev/time#ParseDuration) consisting of numbers and unit suffixes, such as "30s" or "2h45m". Valid time units are "s" (seconds), "m" (minutes), "h" (hours). Setting a timeout for a Delete operation is only applicable if changes are saved into state before the destroy operation occurs.</rdfs:comment>
    <rdfs:domain rdf:resource="http://example.org/onto/class/aws_rekognition_stream_processor"/>
    <rdfs:range rdf:resource="http://www.w3.org/2001/XMLSchema#string"/>
  </owl:DatatypeProperty>
  <owl:DatatypeProperty rdf:about="http://example.org/onto/prop/aws_rekognition_stream_processor_update">
    <rdfs:label>update</rdfs:label>
    <rdfs:comment>A string that can be [parsed as a duration](https://pkg.go.dev/time#ParseDuration) consisting of numbers and unit suffixes, such as "30s" or "2h45m". Valid time units are "s" (seconds), "m" (minutes), "h" (hours).</rdfs:comment>
    <rdfs:domain rdf:resource="http://example.org/onto/class/aws_rekognition_stream_processor"/>
    <rdfs:range rdf:resource="http://www.w3.org/2001/XMLSchema#string"/>
  </owl:DatatypeProperty>
</rdf:RDF>
