<?xml version="1.0" encoding="UTF-8"?>
<rdf:RDF
  xmlns:rdf="http://www.w3.org/1999/02/22-rdf-syntax-ns#"
  xmlns:rdfs="http://www.w3.org/2000/01/rdf-schema#"
  xmlns:owl="http://www.w3.org/2002/07/owl#"
  xmlns:xsd="http://www.w3.org/2001/XMLSchema#"
  xml:base="http://example.org/onto/">
  <owl:Class rdf:about="http://example.org/onto/class/aws_odb_cloud_exadata_infrastructure">
    <rdfs:label>aws_odb_cloud_exadata_infrastructure</rdfs:label>
    <rdfs:comment>Terraform resource for managing exadata infrastructure resource in AWS for Oracle Database@AWS.</rdfs:comment>
  </owl:Class>
  <owl:DatatypeProperty rdf:about="http://example.org/onto/prop/aws_odb_cloud_exadata_infrastructure_activated_storage_count">
    <rdfs:label>activated_storage_count</rdfs:label>
    <rdfs:comment>The number of storage servers requested for the Exadata infrastructure</rdfs:comment>
    <rdfs:domain rdf:resource="http://example.org/onto/class/aws_odb_cloud_exadata_infrastructure"/>
    <rdfs:range rdf:resource="http://www.w3.org/2001/XMLSchema#string"/>
  </owl:DatatypeProperty>
  <owl:DatatypeProperty rdf:about="http://example.org/onto/prop/aws_odb_cloud_exadata_infrastructure_additional_storage_count">
    <rdfs:label>additional_storage_count</rdfs:label>
    <rdfs:comment>The number of storage servers requested for the Exadata infrastructure</rdfs:comment>
    <rdfs:domain rdf:resource="http://example.org/onto/class/aws_odb_cloud_exadata_infrastructure"/>
    <rdfs:range rdf:resource="http://www.w3.org/2001/XMLSchema#string"/>
  </owl:DatatypeProperty>
  <owl:DatatypeProperty rdf:about="http://example.org/onto/prop/aws_odb_cloud_exadata_infrastructure_arn">
    <rdfs:label>arn</rdfs:label>
    <rdfs:domain rdf:resource="http://example.org/onto/class/aws_odb_cloud_exadata_infrastructure"/>
    <rdfs:range rdf:resource="http://www.w3.org/2001/XMLSchema#string"/>
  </owl:DatatypeProperty>
  <owl:DatatypeProperty rdf:about="http://example.org/onto/prop/aws_odb_cloud_exadata_infrastructure_availability_zone">
    <rdfs:label>availability_zone</rdfs:label>
    <rdfs:comment>The name of the Availability Zone (AZ) where the Exadata infrastructure is located. Changing this will force terraform to create new resource</rdfs:comment>
    <rdfs:domain rdf:resource="http://example.org/onto/class/aws_odb_cloud_exadata_infrastructure"/>
    <rdfs:range rdf:resource="http://www.w3.org/2001/XMLSchema#string"/>
  </owl:DatatypeProperty>
  <owl:DatatypeProperty rdf:about="http://example.org/onto/prop/aws_odb_cloud_exadata_infrastructure_availability_zone_id">
    <rdfs:label>availability_zone_id</rdfs:label>
    <rdfs:comment>The AZ ID of the AZ where the Exadata infrastructure is located. Changing this will force terraform to create new resource</rdfs:comment>
    <rdfs:domain rdf:resource="http://example.org/onto/class/aws_odb_cloud_exadata_infrastructure"/>
    <rdfs:range rdf:resource="http://www.w3.org/2001/XMLSchema#string"/>
  </owl:DatatypeProperty>
  <owl:DatatypeProperty rdf:about="http://example.org/onto/prop/aws_odb_cloud_exadata_infrastructure_available_storage_size_in_gbs">
    <rdfs:label>available_storage_size_in_gbs</rdfs:label>
    <rdfs:comment>The amount of available storage, in gigabytes (GB), for the Exadata infrastructure</rdfs:comment>
    <rdfs:domain rdf:resource="http://example.org/onto/class/aws_odb_cloud_exadata_infrastructure"/>
    <rdfs:range rdf:resource="http://www.w3.org/2001/XMLSchema#string"/>
  </owl:DatatypeProperty>
  <owl:DatatypeProperty rdf:about="http://example.org/onto/prop/aws_odb_cloud_exadata_infrastructure_compute_count">
    <rdfs:label>compute_count</rdfs:label>
    <rdfs:comment>The number of compute instances that the Exadata infrastructure is located</rdfs:comment>
    <rdfs:domain rdf:resource="http://example.org/onto/class/aws_odb_cloud_exadata_infrastructure"/>
    <rdfs:range rdf:resource="http://www.w3.org/2001/XMLSchema#string"/>
  </owl:DatatypeProperty>
  <owl:DatatypeProperty rdf:about="http://example.org/onto/prop/aws_odb_cloud_exadata_infrastructure_compute_model">
    <rdfs:label>compute_model</rdfs:label>
    <rdfs:comment>The OCI model compute model used when you create or clone an
  instance: ECPU or OCPU. An ECPU is an abstracted measure of
 compute resources. ECPUs are based on the number of cores
 elastically allocated from a pool of compute and storage servers.
  An OCPU is a legacy physical measure of compute resources. OCPUs
 are based on the physical core of a processor with
  hyper-threading enabled.</rdfs:comment>
    <rdfs:domain rdf:resource="http://example.org/onto/class/aws_odb_cloud_exadata_infrastructure"/>
    <rdfs:range rdf:resource="http://www.w3.org/2001/XMLSchema#string"/>
  </owl:DatatypeProperty>
  <owl:DatatypeProperty rdf:about="http://example.org/onto/prop/aws_odb_cloud_exadata_infrastructure_cpu_count">
    <rdfs:label>cpu_count</rdfs:label>
    <rdfs:comment>The total number of CPU cores that are allocated to the Exadata infrastructure</rdfs:comment>
    <rdfs:domain rdf:resource="http://example.org/onto/class/aws_odb_cloud_exadata_infrastructure"/>
    <rdfs:range rdf:resource="http://www.w3.org/2001/XMLSchema#string"/>
  </owl:DatatypeProperty>
  <owl:DatatypeProperty rdf:about="http://example.org/onto/prop/aws_odb_cloud_exadata_infrastructure_created_at">
    <rdfs:label>created_at</rdfs:label>
    <rdfs:comment>The time when the Exadata infrastructure was created.</rdfs:comment>
    <rdfs:domain rdf:resource="http://example.org/onto/class/aws_odb_cloud_exadata_infrastructure"/>
    <rdfs:range rdf:resource="http://www.w3.org/2001/XMLSchema#string"/>
  </owl:DatatypeProperty>
  <owl:DatatypeProperty rdf:about="http://example.org/onto/prop/aws_odb_cloud_exadata_infrastructure_customer_contacts_to_send_to_oci">
    <rdfs:label>customer_contacts_to_send_to_oci</rdfs:label>
    <rdfs:comment>The email addresses of contacts to receive notification from Oracle about maintenance updates for the Exadata infrastructure. Changing this will force terraform to create new resource</rdfs:comment>
    <rdfs:domain rdf:resource="http://example.org/onto/class/aws_odb_cloud_exadata_infrastructure"/>
    <rdfs:range rdf:resource="http://www.w3.org/2001/XMLSchema#string"/>
  </owl:DatatypeProperty>
  <owl:DatatypeProperty rdf:about="http://example.org/onto/prop/aws_odb_cloud_exadata_infrastructure_data_storage_size_in_tbs">
    <rdfs:label>data_storage_size_in_tbs</rdfs:label>
    <rdfs:comment>The size of the Exadata infrastructure's data disk group, in terabytes (TB)</rdfs:comment>
    <rdfs:domain rdf:resource="http://example.org/onto/class/aws_odb_cloud_exadata_infrastructure"/>
    <rdfs:range rdf:resource="http://www.w3.org/2001/XMLSchema#string"/>
  </owl:DatatypeProperty>
  <owl:DatatypeProperty rdf:about="http://example.org/onto/prop/aws_odb_cloud_exadata_infrastructure_database_server_type">
    <rdfs:label>database_server_type</rdfs:label>
    <rdfs:comment>The database server model type of the Exadata infrastructure. For the list of valid model names, use the ListDbSystemShapes operation</rdfs:comment>
    <rdfs:domain rdf:resource="http://example.org/onto/class/aws_odb_cloud_exadata_infrastructure"/>
    <rdfs:range rdf:resource="http://www.w3.org/2001/XMLSchema#string"/>
  </owl:DatatypeProperty>
  <owl:DatatypeProperty rdf:about="http://example.org/onto/prop/aws_odb_cloud_exadata_infrastructure_db_node_storage_size_in_gbs">
    <rdfs:label>db_node_storage_size_in_gbs</rdfs:label>
    <rdfs:comment>The size of the Exadata infrastructure's local node storage, in gigabytes (GB)</rdfs:comment>
    <rdfs:domain rdf:resource="http://example.org/onto/class/aws_odb_cloud_exadata_infrastructure"/>
    <rdfs:range rdf:resource="http://www.w3.org/2001/XMLSchema#string"/>
  </owl:DatatypeProperty>
  <owl:DatatypeProperty rdf:about="http://example.org/onto/prop/aws_odb_cloud_exadata_infrastructure_db_server_version">
    <rdfs:label>db_server_version</rdfs:label>
    <rdfs:comment>The software version of the database servers (dom0) in the Exadata infrastructure</rdfs:comment>
    <rdfs:domain rdf:resource="http://example.org/onto/class/aws_odb_cloud_exadata_infrastructure"/>
    <rdfs:range rdf:resource="http://www.w3.org/2001/XMLSchema#string"/>
  </owl:DatatypeProperty>
  <owl:DatatypeProperty rdf:about="http://example.org/onto/prop/aws_odb_cloud_exadata_infrastructure_display_name">
    <rdfs:label>display_name</rdfs:label>
    <rdfs:comment>The user-friendly name for the Exadata infrastructure. Changing this will force terraform to create a new resource</rdfs:comment>
    <rdfs:domain rdf:resource="http://example.org/onto/class/aws_odb_cloud_exadata_infrastructure"/>
    <rdfs:range rdf:resource="http://www.w3.org/2001/XMLSchema#string"/>
  </owl:DatatypeProperty>
  <owl:DatatypeProperty rdf:about="http://example.org/onto/prop/aws_odb_cloud_exadata_infrastructure_id">
    <rdfs:label>id</rdfs:label>
    <rdfs:domain rdf:resource="http://example.org/onto/class/aws_odb_cloud_exadata_infrastructure"/>
    <rdfs:range rdf:resource="http://www.w3.org/2001/XMLSchema#string"/>
  </owl:DatatypeProperty>
  <owl:DatatypeProperty rdf:about="http://example.org/onto/prop/aws_odb_cloud_exadata_infrastructure_last_maintenance_run_id">
    <rdfs:label>last_maintenance_run_id</rdfs:label>
    <rdfs:comment>The Oracle Cloud Identifier (OCID) of the last maintenance run for the Exadata infrastructure</rdfs:comment>
    <rdfs:domain rdf:resource="http://example.org/onto/class/aws_odb_cloud_exadata_infrastructure"/>
    <rdfs:range rdf:resource="http://www.w3.org/2001/XMLSchema#string"/>
  </owl:DatatypeProperty>
  <owl:DatatypeProperty rdf:about="http://example.org/onto/prop/aws_odb_cloud_exadata_infrastructure_max_cpu_count">
    <rdfs:label>max_cpu_count</rdfs:label>
    <rdfs:comment>The total number of CPU cores available on the Exadata infrastructure</rdfs:comment>
    <rdfs:domain rdf:resource="http://example.org/onto/class/aws_odb_cloud_exadata_infrastructure"/>
    <rdfs:range rdf:resource="http://www.w3.org/2001/XMLSchema#string"/>
  </owl:DatatypeProperty>
  <owl:DatatypeProperty rdf:about="http://example.org/onto/prop/aws_odb_cloud_exadata_infrastructure_max_data_storage_in_tbs">
    <rdfs:label>max_data_storage_in_tbs</rdfs:label>
    <rdfs:comment>The total amount of data disk group storage, in terabytes (TB), that's available on the Exadata infrastructure</rdfs:comment>
    <rdfs:domain rdf:resource="http://example.org/onto/class/aws_odb_cloud_exadata_infrastructure"/>
    <rdfs:range rdf:resource="http://www.w3.org/2001/XMLSchema#string"/>
  </owl:DatatypeProperty>
  <owl:DatatypeProperty rdf:about="http://example.org/onto/prop/aws_odb_cloud_exadata_infrastructure_max_db_node_storage_size_in_gbs">
    <rdfs:label>max_db_node_storage_size_in_gbs</rdfs:label>
    <rdfs:comment>The total amount of local node storage, in gigabytes (GB), that's available on the Exadata infrastructure</rdfs:comment>
    <rdfs:domain rdf:resource="http://example.org/onto/class/aws_odb_cloud_exadata_infrastructure"/>
    <rdfs:range rdf:resource="http://www.w3.org/2001/XMLSchema#string"/>
  </owl:DatatypeProperty>
  <owl:DatatypeProperty rdf:about="http://example.org/onto/prop/aws_odb_cloud_exadata_infrastructure_max_memory_in_gbs">
    <rdfs:label>max_memory_in_gbs</rdfs:label>
    <rdfs:comment>The total amount of memory in gigabytes (GB) available on the Exadata infrastructure</rdfs:comment>
    <rdfs:domain rdf:resource="http://example.org/onto/class/aws_odb_cloud_exadata_infrastructure"/>
    <rdfs:range rdf:resource="http://www.w3.org/2001/XMLSchema#string"/>
  </owl:DatatypeProperty>
  <owl:DatatypeProperty rdf:about="http://example.org/onto/prop/aws_odb_cloud_exadata_infrastructure_memory_size_in_gbs">
    <rdfs:label>memory_size_in_gbs</rdfs:label>
    <rdfs:comment>The amount of memory, in gigabytes (GB), that's allocated on the Exadata infrastructure</rdfs:comment>
    <rdfs:domain rdf:resource="http://example.org/onto/class/aws_odb_cloud_exadata_infrastructure"/>
    <rdfs:range rdf:resource="http://www.w3.org/2001/XMLSchema#string"/>
  </owl:DatatypeProperty>
  <owl:DatatypeProperty rdf:about="http://example.org/onto/prop/aws_odb_cloud_exadata_infrastructure_monthly_db_server_version">
    <rdfs:label>monthly_db_server_version</rdfs:label>
    <rdfs:comment>The monthly software version of the database servers in the Exadata infrastructure</rdfs:comment>
    <rdfs:domain rdf:resource="http://example.org/onto/class/aws_odb_cloud_exadata_infrastructure"/>
    <rdfs:range rdf:resource="http://www.w3.org/2001/XMLSchema#string"/>
  </owl:DatatypeProperty>
  <owl:DatatypeProperty rdf:about="http://example.org/onto/prop/aws_odb_cloud_exadata_infrastructure_monthly_storage_server_version">
    <rdfs:label>monthly_storage_server_version</rdfs:label>
    <rdfs:comment>The monthly software version of the storage servers installed on the Exadata infrastructure</rdfs:comment>
    <rdfs:domain rdf:resource="http://example.org/onto/class/aws_odb_cloud_exadata_infrastructure"/>
    <rdfs:range rdf:resource="http://www.w3.org/2001/XMLSchema#string"/>
  </owl:DatatypeProperty>
  <owl:DatatypeProperty rdf:about="http://example.org/onto/prop/aws_odb_cloud_exadata_infrastructure_next_maintenance_run_id">
    <rdfs:label>next_maintenance_run_id</rdfs:label>
    <rdfs:comment>The OCID of the next maintenance run for the Exadata infrastructure</rdfs:comment>
    <rdfs:domain rdf:resource="http://example.org/onto/class/aws_odb_cloud_exadata_infrastructure"/>
    <rdfs:range rdf:resource="http://www.w3.org/2001/XMLSchema#string"/>
  </owl:DatatypeProperty>
  <owl:DatatypeProperty rdf:about="http://example.org/onto/prop/aws_odb_cloud_exadata_infrastructure_oci_resource_anchor_name">
    <rdfs:label>oci_resource_anchor_name</rdfs:label>
    <rdfs:comment>The name of the OCI resource anchor for the Exadata infrastructure</rdfs:comment>
    <rdfs:domain rdf:resource="http://example.org/onto/class/aws_odb_cloud_exadata_infrastructure"/>
    <rdfs:range rdf:resource="http://www.w3.org/2001/XMLSchema#string"/>
  </owl:DatatypeProperty>
  <owl:DatatypeProperty rdf:about="http://example.org/onto/prop/aws_odb_cloud_exadata_infrastructure_oci_url">
    <rdfs:label>oci_url</rdfs:label>
    <rdfs:comment>The HTTPS link to the Exadata infrastructure in OCI</rdfs:comment>
    <rdfs:domain rdf:resource="http://example.org/onto/class/aws_odb_cloud_exadata_infrastructure"/>
    <rdfs:range rdf:resource="http://www.w3.org/2001/XMLSchema#string"/>
  </owl:DatatypeProperty>
  <owl:DatatypeProperty rdf:about="http://example.org/onto/prop/aws_odb_cloud_exadata_infrastructure_ocid">
    <rdfs:label>ocid</rdfs:label>
    <rdfs:comment>The OCID of the Exadata infrastructure</rdfs:comment>
    <rdfs:domain rdf:resource="http://example.org/onto/class/aws_odb_cloud_exadata_infrastructure"/>
    <rdfs:range rdf:resource="http://www.w3.org/2001/XMLSchema#string"/>
  </owl:DatatypeProperty>
  <owl:DatatypeProperty rdf:about="http://example.org/onto/prop/aws_odb_cloud_exadata_infrastructure_percent_progress">
    <rdfs:label>percent_progress</rdfs:label>
    <rdfs:comment>The amount of progress made on the current operation on the Exadata infrastructure, expressed as a percentage</rdfs:comment>
    <rdfs:domain rdf:resource="http://example.org/onto/class/aws_odb_cloud_exadata_infrastructure"/>
    <rdfs:range rdf:resource="http://www.w3.org/2001/XMLSchema#string"/>
  </owl:DatatypeProperty>
  <owl:DatatypeProperty rdf:about="http://example.org/onto/prop/aws_odb_cloud_exadata_infrastructure_region">
    <rdfs:label>region</rdfs:label>
    <rdfs:comment>Region where this resource will be [managed](https://docs.aws.amazon.com/general/latest/gr/rande.html#regional-endpoints). Defaults to the Region set in the [provider configuration](https://registry.terraform.io/providers/hashicorp/aws/latest/docs#aws-configuration-reference).</rdfs:comment>
    <rdfs:domain rdf:resource="http://example.org/onto/class/aws_odb_cloud_exadata_infrastructure"/>
    <rdfs:range rdf:resource="http://www.w3.org/2001/XMLSchema#string"/>
  </owl:DatatypeProperty>
  <owl:DatatypeProperty rdf:about="http://example.org/onto/prop/aws_odb_cloud_exadata_infrastructure_shape">
    <rdfs:label>shape</rdfs:label>
    <rdfs:comment>The model name of the Exadata infrastructure. Changing this will force terraform to create new resource</rdfs:comment>
    <rdfs:domain rdf:resource="http://example.org/onto/class/aws_odb_cloud_exadata_infrastructure"/>
    <rdfs:range rdf:resource="http://www.w3.org/2001/XMLSchema#string"/>
  </owl:DatatypeProperty>
  <owl:DatatypeProperty rdf:about="http://example.org/onto/prop/aws_odb_cloud_exadata_infrastructure_status">
    <rdfs:label>status</rdfs:label>
    <rdfs:comment>The current status of the Exadata infrastructure</rdfs:comment>
    <rdfs:domain rdf:resource="http://example.org/onto/class/aws_odb_cloud_exadata_infrastructure"/>
    <rdfs:range rdf:resource="http://www.w3.org/2001/XMLSchema#string"/>
  </owl:DatatypeProperty>
  <owl:DatatypeProperty rdf:about="http://example.org/onto/prop/aws_odb_cloud_exadata_infrastructure_status_reason">
    <rdfs:label>status_reason</rdfs:label>
    <rdfs:comment>Additional information about the status of the Exadata infrastructure</rdfs:comment>
    <rdfs:domain rdf:resource="http://example.org/onto/class/aws_odb_cloud_exadata_infrastructure"/>
    <rdfs:range rdf:resource="http://www.w3.org/2001/XMLSchema#string"/>
  </owl:DatatypeProperty>
  <owl:DatatypeProperty rdf:about="http://example.org/onto/prop/aws_odb_cloud_exadata_infrastructure_storage_count">
    <rdfs:label>storage_count</rdfs:label>
    <rdfs:comment>TThe number of storage servers that are activated for the Exadata infrastructure</rdfs:comment>
    <rdfs:domain rdf:resource="http://example.org/onto/class/aws_odb_cloud_exadata_infrastructure"/>
    <rdfs:range rdf:resource="http://www.w3.org/2001/XMLSchema#string"/>
  </owl:DatatypeProperty>
  <owl:DatatypeProperty rdf:about="http://example.org/onto/prop/aws_odb_cloud_exadata_infrastructure_storage_server_type">
    <rdfs:label>storage_server_type</rdfs:label>
    <rdfs:comment>The storage server model type of the Exadata infrastructure. For the list of valid model names, use the ListDbSystemShapes operation</rdfs:comment>
    <rdfs:domain rdf:resource="http://example.org/onto/class/aws_odb_cloud_exadata_infrastructure"/>
    <rdfs:range rdf:resource="http://www.w3.org/2001/XMLSchema#string"/>
  </owl:DatatypeProperty>
  <owl:DatatypeProperty rdf:about="http://example.org/onto/prop/aws_odb_cloud_exadata_infrastructure_storage_server_version">
    <rdfs:label>storage_server_version</rdfs:label>
    <rdfs:comment>The software version of the storage servers on the Exadata infrastructure.</rdfs:comment>
    <rdfs:domain rdf:resource="http://example.org/onto/class/aws_odb_cloud_exadata_infrastructure"/>
    <rdfs:range rdf:resource="http://www.w3.org/2001/XMLSchema#string"/>
  </owl:DatatypeProperty>
  <owl:DatatypeProperty rdf:about="http://example.org/onto/prop/aws_odb_cloud_exadata_infrastructure_tags">
    <rdfs:label>tags</rdfs:label>
    <rdfs:domain rdf:resource="http://example.org/onto/class/aws_odb_cloud_exadata_infrastructure"/>
    <rdfs:range rdf:resource="http://www.w3.org/2001/XMLSchema#string"/>
  </owl:DatatypeProperty>
  <owl:DatatypeProperty rdf:about="http://example.org/onto/prop/aws_odb_cloud_exadata_infrastructure_tags_all">
    <rdfs:label>tags_all</rdfs:label>
    <rdfs:domain rdf:resource="http://example.org/onto/class/aws_odb_cloud_exadata_infrastructure"/>
    <rdfs:range rdf:resource="http://www.w3.org/2001/XMLSchema#string"/>
  </owl:DatatypeProperty>
  <owl:DatatypeProperty rdf:about="http://example.org/onto/prop/aws_odb_cloud_exadata_infrastructure_total_storage_size_in_gbs">
    <rdfs:label>total_storage_size_in_gbs</rdfs:label>
    <rdfs:comment>The total amount of storage, in gigabytes (GB), on the Exadata infrastructure.</rdfs:comment>
    <rdfs:domain rdf:resource="http://example.org/onto/class/aws_odb_cloud_exadata_infrastructure"/>
    <rdfs:range rdf:resource="http://www.w3.org/2001/XMLSchema#string"/>
  </owl:DatatypeProperty>
  <owl:DatatypeProperty rdf:about="http://example.org/onto/prop/aws_odb_cloud_exadata_infrastructure_custom_action_timeout_in_mins">
    <rdfs:label>custom_action_timeout_in_mins</rdfs:label>
    <rdfs:domain rdf:resource="http://example.org/onto/class/aws_odb_cloud_exadata_infrastructure"/>
    <rdfs:range rdf:resource="http://www.w3.org/2001/XMLSchema#string"/>
  </owl:DatatypeProperty>
  <owl:DatatypeProperty rdf:about="http://example.org/onto/prop/aws_odb_cloud_exadata_infrastructure_days_of_week">
    <rdfs:label>days_of_week</rdfs:label>
    <rdfs:domain rdf:resource="http://example.org/onto/class/aws_odb_cloud_exadata_infrastructure"/>
    <rdfs:range rdf:resource="http://www.w3.org/2001/XMLSchema#string"/>
  </owl:DatatypeProperty>
  <owl:DatatypeProperty rdf:about="http://example.org/onto/prop/aws_odb_cloud_exadata_infrastructure_hours_of_day">
    <rdfs:label>hours_of_day</rdfs:label>
    <rdfs:domain rdf:resource="http://example.org/onto/class/aws_odb_cloud_exadata_infrastructure"/>
    <rdfs:range rdf:resource="http://www.w3.org/2001/XMLSchema#string"/>
  </owl:DatatypeProperty>
  <owl:DatatypeProperty rdf:about="http://example.org/onto/prop/aws_odb_cloud_exadata_infrastructure_is_custom_action_timeout_enabled">
    <rdfs:label>is_custom_action_timeout_enabled</rdfs:label>
    <rdfs:domain rdf:resource="http://example.org/onto/class/aws_odb_cloud_exadata_infrastructure"/>
    <rdfs:range rdf:resource="http://www.w3.org/2001/XMLSchema#string"/>
  </owl:DatatypeProperty>
  <owl:DatatypeProperty rdf:about="http://example.org/onto/prop/aws_odb_cloud_exadata_infrastructure_lead_time_in_weeks">
    <rdfs:label>lead_time_in_weeks</rdfs:label>
    <rdfs:domain rdf:resource="http://example.org/onto/class/aws_odb_cloud_exadata_infrastructure"/>
    <rdfs:range rdf:resource="http://www.w3.org/2001/XMLSchema#string"/>
  </owl:DatatypeProperty>
  <owl:DatatypeProperty rdf:about="http://example.org/onto/prop/aws_odb_cloud_exadata_infrastructure_months">
    <rdfs:label>months</rdfs:label>
    <rdfs:domain rdf:resource="http://example.org/onto/class/aws_odb_cloud_exadata_infrastructure"/>
    <rdfs:range rdf:resource="http://www.w3.org/2001/XMLSchema#string"/>
  </owl:DatatypeProperty>
  <owl:DatatypeProperty rdf:about="http://example.org/onto/prop/aws_odb_cloud_exadata_infrastructure_patching_mode">
    <rdfs:label>patching_mode</rdfs:label>
    <rdfs:domain rdf:resource="http://example.org/onto/class/aws_odb_cloud_exadata_infrastructure"/>
    <rdfs:range rdf:resource="http://www.w3.org/2001/XMLSchema#string"/>
  </owl:DatatypeProperty>
  <owl:DatatypeProperty rdf:about="http://example.org/onto/prop/aws_odb_cloud_exadata_infrastructure_preference">
    <rdfs:label>preference</rdfs:label>
    <rdfs:domain rdf:resource="http://example.org/onto/class/aws_odb_cloud_exadata_infrastructure"/>
    <rdfs:range rdf:resource="http://www.w3.org/2001/XMLSchema#string"/>
  </owl:DatatypeProperty>
  <owl:DatatypeProperty rdf:about="http://example.org/onto/prop/aws_odb_cloud_exadata_infrastructure_weeks_of_month">
    <rdfs:label>weeks_of_month</rdfs:label>
    <rdfs:domain rdf:resource="http://example.org/onto/class/aws_odb_cloud_exadata_infrastructure"/>
    <rdfs:range rdf:resource="http://www.w3.org/2001/XMLSchema#string"/>
  </owl:DatatypeProperty>
  <owl:DatatypeProperty rdf:about="http://example.org/onto/prop/aws_odb_cloud_exadata_infrastructure_create">
    <rdfs:label>create</rdfs:label>
    <rdfs:comment>A string that can be [parsed as a duration](https://pkg.go.dev/time#ParseDuration) consisting of numbers and unit suffixes, such as "30s" or "2h45m". Valid time units are "s" (seconds), "m" (minutes), "h" (hours).</rdfs:comment>
    <rdfs:domain rdf:resource="http://example.org/onto/class/aws_odb_cloud_exadata_infrastructure"/>
    <rdfs:range rdf:resource="http://www.w3.org/2001/XMLSchema#string"/>
  </owl:DatatypeProperty>
  <owl:DatatypeProperty rdf:about="http://example.org/onto/prop/aws_odb_cloud_exadata_infrastructure_delete">
    <rdfs:label>delete</rdfs:label>
    <rdfs:comment>A string that can be [parsed as a duration](https://pkg.go.dev/time#ParseDuration) consisting of numbers and unit suffixes, such as "30s" or "2h45m". Valid time units are "s" (seconds), "m" (minutes), "h" (hours). Setting a timeout for a Delete operation is only applicable if changes are saved into state before the destroy operation occurs.</rdfs:comment>
    <rdfs:domain rdf:resource="http://example.org/onto/class/aws_odb_cloud_exadata_infrastructure"/>
    <rdfs:range rdf:resource="http://www.w3.org/2001/XMLSchema#string"/>
  </owl:DatatypeProperty>
  <owl:DatatypeProperty rdf:about="http://example.org/onto/prop/aws_odb_cloud_exadata_infrastructure_update">
    <rdfs:label>update</rdfs:label>
    <rdfs:comment>A string that can be [parsed as a duration](https://pkg.go.dev/time#ParseDuration) consisting of numbers and unit suffixes, such as "30s" or "2h45m". Valid time units are "s" (seconds), "m" (minutes), "h" (hours).</rdfs:comment>
    <rdfs:domain rdf:resource="http://example.org/onto/class/aws_odb_cloud_exadata_infrastructure"/>
    <rdfs:range rdf:resource="http://www.w3.org/2001/XMLSchema#string"/>
  </owl:DatatypeProperty>
</rdf:RDF>
