<?xml version="1.0" encoding="UTF-8"?>
<rdf:RDF
  xmlns:rdf="http://www.w3.org/1999/02/22-rdf-syntax-ns#"
  xmlns:rdfs="http://www.w3.org/2000/01/rdf-schema#"
  xmlns:owl="http://www.w3.org/2002/07/owl#"
  xmlns:xsd="http://www.w3.org/2001/XMLSchema#"
  xml:base="http://example.org/onto/">
  <owl:Class rdf:about="http://example.org/onto/class/azurerm_linux_function_app">
    <rdfs:label>azurerm_linux_function_app</rdfs:label>
  </owl:Class>
  <owl:DatatypeProperty rdf:about="http://example.org/onto/prop/azurerm_linux_function_app_app_settings">
    <rdfs:label>app_settings</rdfs:label>
    <rdfs:comment>A map of key-value pairs for [App Settings](https://docs.microsoft.com/en-us/azure/azure-functions/functions-app-settings) and custom values.</rdfs:comment>
    <rdfs:domain rdf:resource="http://example.org/onto/class/azurerm_linux_function_app"/>
    <rdfs:range rdf:resource="http://www.w3.org/2001/XMLSchema#string"/>
  </owl:DatatypeProperty>
  <owl:DatatypeProperty rdf:about="http://example.org/onto/prop/azurerm_linux_function_app_builtin_logging_enabled">
    <rdfs:label>builtin_logging_enabled</rdfs:label>
    <rdfs:comment>Should built in logging be enabled. Configures `AzureWebJobsDashboard` app setting based on the configured storage setting</rdfs:comment>
    <rdfs:domain rdf:resource="http://example.org/onto/class/azurerm_linux_function_app"/>
    <rdfs:range rdf:resource="http://www.w3.org/2001/XMLSchema#string"/>
  </owl:DatatypeProperty>
  <owl:DatatypeProperty rdf:about="http://example.org/onto/prop/azurerm_linux_function_app_client_certificate_enabled">
    <rdfs:label>client_certificate_enabled</rdfs:label>
    <rdfs:comment>Should the function app use Client Certificates</rdfs:comment>
    <rdfs:domain rdf:resource="http://example.org/onto/class/azurerm_linux_function_app"/>
    <rdfs:range rdf:resource="http://www.w3.org/2001/XMLSchema#string"/>
  </owl:DatatypeProperty>
  <owl:DatatypeProperty rdf:about="http://example.org/onto/prop/azurerm_linux_function_app_client_certificate_exclusion_paths">
    <rdfs:label>client_certificate_exclusion_paths</rdfs:label>
    <rdfs:comment>Paths to exclude when using client certificates, separated by ;</rdfs:comment>
    <rdfs:domain rdf:resource="http://example.org/onto/class/azurerm_linux_function_app"/>
    <rdfs:range rdf:resource="http://www.w3.org/2001/XMLSchema#string"/>
  </owl:DatatypeProperty>
  <owl:DatatypeProperty rdf:about="http://example.org/onto/prop/azurerm_linux_function_app_client_certificate_mode">
    <rdfs:label>client_certificate_mode</rdfs:label>
    <rdfs:comment>The mode of the Function App's client certificates requirement for incoming requests. Possible values are `Required`, `Optional`, and `OptionalInteractiveUser`</rdfs:comment>
    <rdfs:domain rdf:resource="http://example.org/onto/class/azurerm_linux_function_app"/>
    <rdfs:range rdf:resource="http://www.w3.org/2001/XMLSchema#string"/>
  </owl:DatatypeProperty>
  <owl:DatatypeProperty rdf:about="http://example.org/onto/prop/azurerm_linux_function_app_content_share_force_disabled">
    <rdfs:label>content_share_force_disabled</rdfs:label>
    <rdfs:comment>Force disable the content share settings.</rdfs:comment>
    <rdfs:domain rdf:resource="http://example.org/onto/class/azurerm_linux_function_app"/>
    <rdfs:range rdf:resource="http://www.w3.org/2001/XMLSchema#string"/>
  </owl:DatatypeProperty>
  <owl:DatatypeProperty rdf:about="http://example.org/onto/prop/azurerm_linux_function_app_custom_domain_verification_id">
    <rdfs:label>custom_domain_verification_id</rdfs:label>
    <rdfs:domain rdf:resource="http://example.org/onto/class/azurerm_linux_function_app"/>
    <rdfs:range rdf:resource="http://www.w3.org/2001/XMLSchema#string"/>
  </owl:DatatypeProperty>
  <owl:DatatypeProperty rdf:about="http://example.org/onto/prop/azurerm_linux_function_app_daily_memory_time_quota">
    <rdfs:label>daily_memory_time_quota</rdfs:label>
    <rdfs:comment>The amount of memory in gigabyte-seconds that your application is allowed to consume per day. Setting this value only affects function apps in Consumption Plans.</rdfs:comment>
    <rdfs:domain rdf:resource="http://example.org/onto/class/azurerm_linux_function_app"/>
    <rdfs:range rdf:resource="http://www.w3.org/2001/XMLSchema#string"/>
  </owl:DatatypeProperty>
  <owl:DatatypeProperty rdf:about="http://example.org/onto/prop/azurerm_linux_function_app_default_hostname">
    <rdfs:label>default_hostname</rdfs:label>
    <rdfs:domain rdf:resource="http://example.org/onto/class/azurerm_linux_function_app"/>
    <rdfs:range rdf:resource="http://www.w3.org/2001/XMLSchema#string"/>
  </owl:DatatypeProperty>
  <owl:DatatypeProperty rdf:about="http://example.org/onto/prop/azurerm_linux_function_app_enabled">
    <rdfs:label>enabled</rdfs:label>
    <rdfs:comment>Is the Linux Function App enabled.</rdfs:comment>
    <rdfs:domain rdf:resource="http://example.org/onto/class/azurerm_linux_function_app"/>
    <rdfs:range rdf:resource="http://www.w3.org/2001/XMLSchema#string"/>
  </owl:DatatypeProperty>
  <owl:DatatypeProperty rdf:about="http://example.org/onto/prop/azurerm_linux_function_app_ftp_publish_basic_authentication_enabled">
    <rdfs:label>ftp_publish_basic_authentication_enabled</rdfs:label>
    <rdfs:domain rdf:resource="http://example.org/onto/class/azurerm_linux_function_app"/>
    <rdfs:range rdf:resource="http://www.w3.org/2001/XMLSchema#string"/>
  </owl:DatatypeProperty>
  <owl:DatatypeProperty rdf:about="http://example.org/onto/prop/azurerm_linux_function_app_functions_extension_version">
    <rdfs:label>functions_extension_version</rdfs:label>
    <rdfs:comment>The runtime version associated with the Function App.</rdfs:comment>
    <rdfs:domain rdf:resource="http://example.org/onto/class/azurerm_linux_function_app"/>
    <rdfs:range rdf:resource="http://www.w3.org/2001/XMLSchema#string"/>
  </owl:DatatypeProperty>
  <owl:DatatypeProperty rdf:about="http://example.org/onto/prop/azurerm_linux_function_app_hosting_environment_id">
    <rdfs:label>hosting_environment_id</rdfs:label>
    <rdfs:domain rdf:resource="http://example.org/onto/class/azurerm_linux_function_app"/>
    <rdfs:range rdf:resource="http://www.w3.org/2001/XMLSchema#string"/>
  </owl:DatatypeProperty>
  <owl:DatatypeProperty rdf:about="http://example.org/onto/prop/azurerm_linux_function_app_https_only">
    <rdfs:label>https_only</rdfs:label>
    <rdfs:comment>Can the Function App only be accessed via HTTPS?</rdfs:comment>
    <rdfs:domain rdf:resource="http://example.org/onto/class/azurerm_linux_function_app"/>
    <rdfs:range rdf:resource="http://www.w3.org/2001/XMLSchema#string"/>
  </owl:DatatypeProperty>
  <owl:DatatypeProperty rdf:about="http://example.org/onto/prop/azurerm_linux_function_app_id">
    <rdfs:label>id</rdfs:label>
    <rdfs:domain rdf:resource="http://example.org/onto/class/azurerm_linux_function_app"/>
    <rdfs:range rdf:resource="http://www.w3.org/2001/XMLSchema#string"/>
  </owl:DatatypeProperty>
  <owl:DatatypeProperty rdf:about="http://example.org/onto/prop/azurerm_linux_function_app_key_vault_reference_identity_id">
    <rdfs:label>key_vault_reference_identity_id</rdfs:label>
    <rdfs:comment>The User Assigned Identity to use for Key Vault access.</rdfs:comment>
    <rdfs:domain rdf:resource="http://example.org/onto/class/azurerm_linux_function_app"/>
    <rdfs:range rdf:resource="http://www.w3.org/2001/XMLSchema#string"/>
  </owl:DatatypeProperty>
  <owl:DatatypeProperty rdf:about="http://example.org/onto/prop/azurerm_linux_function_app_kind">
    <rdfs:label>kind</rdfs:label>
    <rdfs:domain rdf:resource="http://example.org/onto/class/azurerm_linux_function_app"/>
    <rdfs:range rdf:resource="http://www.w3.org/2001/XMLSchema#string"/>
  </owl:DatatypeProperty>
  <owl:DatatypeProperty rdf:about="http://example.org/onto/prop/azurerm_linux_function_app_location">
    <rdfs:label>location</rdfs:label>
    <rdfs:domain rdf:resource="http://example.org/onto/class/azurerm_linux_function_app"/>
    <rdfs:range rdf:resource="http://www.w3.org/2001/XMLSchema#string"/>
  </owl:DatatypeProperty>
  <owl:DatatypeProperty rdf:about="http://example.org/onto/prop/azurerm_linux_function_app_name">
    <rdfs:label>name</rdfs:label>
    <rdfs:comment>Specifies the name of the Function App.</rdfs:comment>
    <rdfs:domain rdf:resource="http://example.org/onto/class/azurerm_linux_function_app"/>
    <rdfs:range rdf:resource="http://www.w3.org/2001/XMLSchema#string"/>
  </owl:DatatypeProperty>
  <owl:DatatypeProperty rdf:about="http://example.org/onto/prop/azurerm_linux_function_app_outbound_ip_address_list">
    <rdfs:label>outbound_ip_address_list</rdfs:label>
    <rdfs:domain rdf:resource="http://example.org/onto/class/azurerm_linux_function_app"/>
    <rdfs:range rdf:resource="http://www.w3.org/2001/XMLSchema#string"/>
  </owl:DatatypeProperty>
  <owl:DatatypeProperty rdf:about="http://example.org/onto/prop/azurerm_linux_function_app_outbound_ip_addresses">
    <rdfs:label>outbound_ip_addresses</rdfs:label>
    <rdfs:domain rdf:resource="http://example.org/onto/class/azurerm_linux_function_app"/>
    <rdfs:range rdf:resource="http://www.w3.org/2001/XMLSchema#string"/>
  </owl:DatatypeProperty>
  <owl:DatatypeProperty rdf:about="http://example.org/onto/prop/azurerm_linux_function_app_possible_outbound_ip_address_list">
    <rdfs:label>possible_outbound_ip_address_list</rdfs:label>
    <rdfs:domain rdf:resource="http://example.org/onto/class/azurerm_linux_function_app"/>
    <rdfs:range rdf:resource="http://www.w3.org/2001/XMLSchema#string"/>
  </owl:DatatypeProperty>
  <owl:DatatypeProperty rdf:about="http://example.org/onto/prop/azurerm_linux_function_app_possible_outbound_ip_addresses">
    <rdfs:label>possible_outbound_ip_addresses</rdfs:label>
    <rdfs:domain rdf:resource="http://example.org/onto/class/azurerm_linux_function_app"/>
    <rdfs:range rdf:resource="http://www.w3.org/2001/XMLSchema#string"/>
  </owl:DatatypeProperty>
  <owl:DatatypeProperty rdf:about="http://example.org/onto/prop/azurerm_linux_function_app_public_network_access_enabled">
    <rdfs:label>public_network_access_enabled</rdfs:label>
    <rdfs:domain rdf:resource="http://example.org/onto/class/azurerm_linux_function_app"/>
    <rdfs:range rdf:resource="http://www.w3.org/2001/XMLSchema#string"/>
  </owl:DatatypeProperty>
  <owl:DatatypeProperty rdf:about="http://example.org/onto/prop/azurerm_linux_function_app_resource_group_name">
    <rdfs:label>resource_group_name</rdfs:label>
    <rdfs:domain rdf:resource="http://example.org/onto/class/azurerm_linux_function_app"/>
    <rdfs:range rdf:resource="http://www.w3.org/2001/XMLSchema#string"/>
  </owl:DatatypeProperty>
  <owl:DatatypeProperty rdf:about="http://example.org/onto/prop/azurerm_linux_function_app_service_plan_id">
    <rdfs:label>service_plan_id</rdfs:label>
    <rdfs:comment>The ID of the App Service Plan within which to create this Function App</rdfs:comment>
    <rdfs:domain rdf:resource="http://example.org/onto/class/azurerm_linux_function_app"/>
    <rdfs:range rdf:resource="http://www.w3.org/2001/XMLSchema#string"/>
  </owl:DatatypeProperty>
  <owl:DatatypeProperty rdf:about="http://example.org/onto/prop/azurerm_linux_function_app_site_credential">
    <rdfs:label>site_credential</rdfs:label>
    <rdfs:domain rdf:resource="http://example.org/onto/class/azurerm_linux_function_app"/>
    <rdfs:range rdf:resource="http://www.w3.org/2001/XMLSchema#string"/>
  </owl:DatatypeProperty>
  <owl:DatatypeProperty rdf:about="http://example.org/onto/prop/azurerm_linux_function_app_storage_account_access_key">
    <rdfs:label>storage_account_access_key</rdfs:label>
    <rdfs:comment>The access key which will be used to access the storage account for the Function App.</rdfs:comment>
    <rdfs:domain rdf:resource="http://example.org/onto/class/azurerm_linux_function_app"/>
    <rdfs:range rdf:resource="http://www.w3.org/2001/XMLSchema#string"/>
  </owl:DatatypeProperty>
  <owl:DatatypeProperty rdf:about="http://example.org/onto/prop/azurerm_linux_function_app_storage_account_name">
    <rdfs:label>storage_account_name</rdfs:label>
    <rdfs:comment>The backend storage account name which will be used by this Function App.</rdfs:comment>
    <rdfs:domain rdf:resource="http://example.org/onto/class/azurerm_linux_function_app"/>
    <rdfs:range rdf:resource="http://www.w3.org/2001/XMLSchema#string"/>
  </owl:DatatypeProperty>
  <owl:DatatypeProperty rdf:about="http://example.org/onto/prop/azurerm_linux_function_app_storage_key_vault_secret_id">
    <rdfs:label>storage_key_vault_secret_id</rdfs:label>
    <rdfs:comment>The Key Vault Secret ID, including version, that contains the Connection String to connect to the storage account for this Function App.</rdfs:comment>
    <rdfs:domain rdf:resource="http://example.org/onto/class/azurerm_linux_function_app"/>
    <rdfs:range rdf:resource="http://www.w3.org/2001/XMLSchema#string"/>
  </owl:DatatypeProperty>
  <owl:DatatypeProperty rdf:about="http://example.org/onto/prop/azurerm_linux_function_app_storage_uses_managed_identity">
    <rdfs:label>storage_uses_managed_identity</rdfs:label>
    <rdfs:comment>Should the Function App use its Managed Identity to access storage?</rdfs:comment>
    <rdfs:domain rdf:resource="http://example.org/onto/class/azurerm_linux_function_app"/>
    <rdfs:range rdf:resource="http://www.w3.org/2001/XMLSchema#string"/>
  </owl:DatatypeProperty>
  <owl:DatatypeProperty rdf:about="http://example.org/onto/prop/azurerm_linux_function_app_tags">
    <rdfs:label>tags</rdfs:label>
    <rdfs:domain rdf:resource="http://example.org/onto/class/azurerm_linux_function_app"/>
    <rdfs:range rdf:resource="http://www.w3.org/2001/XMLSchema#string"/>
  </owl:DatatypeProperty>
  <owl:DatatypeProperty rdf:about="http://example.org/onto/prop/azurerm_linux_function_app_virtual_network_backup_restore_enabled">
    <rdfs:label>virtual_network_backup_restore_enabled</rdfs:label>
    <rdfs:domain rdf:resource="http://example.org/onto/class/azurerm_linux_function_app"/>
    <rdfs:range rdf:resource="http://www.w3.org/2001/XMLSchema#string"/>
  </owl:DatatypeProperty>
  <owl:DatatypeProperty rdf:about="http://example.org/onto/prop/azurerm_linux_function_app_virtual_network_subnet_id">
    <rdfs:label>virtual_network_subnet_id</rdfs:label>
    <rdfs:domain rdf:resource="http://example.org/onto/class/azurerm_linux_function_app"/>
    <rdfs:range rdf:resource="http://www.w3.org/2001/XMLSchema#string"/>
  </owl:DatatypeProperty>
  <owl:DatatypeProperty rdf:about="http://example.org/onto/prop/azurerm_linux_function_app_vnet_image_pull_enabled">
    <rdfs:label>vnet_image_pull_enabled</rdfs:label>
    <rdfs:comment>Is container image pull over virtual network enabled? Defaults to `false`.</rdfs:comment>
    <rdfs:domain rdf:resource="http://example.org/onto/class/azurerm_linux_function_app"/>
    <rdfs:range rdf:resource="http://www.w3.org/2001/XMLSchema#string"/>
  </owl:DatatypeProperty>
  <owl:DatatypeProperty rdf:about="http://example.org/onto/prop/azurerm_linux_function_app_webdeploy_publish_basic_authentication_enabled">
    <rdfs:label>webdeploy_publish_basic_authentication_enabled</rdfs:label>
    <rdfs:domain rdf:resource="http://example.org/onto/class/azurerm_linux_function_app"/>
    <rdfs:range rdf:resource="http://www.w3.org/2001/XMLSchema#string"/>
  </owl:DatatypeProperty>
  <owl:DatatypeProperty rdf:about="http://example.org/onto/prop/azurerm_linux_function_app_zip_deploy_file">
    <rdfs:label>zip_deploy_file</rdfs:label>
    <rdfs:comment>The local path and filename of the Zip packaged application to deploy to this Linux Function App. **Note:** Using this value requires either `WEBSITE_RUN_FROM_PACKAGE=1` or `SCM_DO_BUILD_DURING_DEPLOYMENT=true` to be set on the App in `app_settings`.</rdfs:comment>
    <rdfs:domain rdf:resource="http://example.org/onto/class/azurerm_linux_function_app"/>
    <rdfs:range rdf:resource="http://www.w3.org/2001/XMLSchema#string"/>
  </owl:DatatypeProperty>
  <owl:DatatypeProperty rdf:about="http://example.org/onto/prop/azurerm_linux_function_app_additional_login_parameters">
    <rdfs:label>additional_login_parameters</rdfs:label>
    <rdfs:comment>Specifies a map of Login Parameters to send to the OpenID Connect authorization endpoint when a user logs in.</rdfs:comment>
    <rdfs:domain rdf:resource="http://example.org/onto/class/azurerm_linux_function_app"/>
    <rdfs:range rdf:resource="http://www.w3.org/2001/XMLSchema#string"/>
  </owl:DatatypeProperty>
  <owl:DatatypeProperty rdf:about="http://example.org/onto/prop/azurerm_linux_function_app_allowed_external_redirect_urls">
    <rdfs:label>allowed_external_redirect_urls</rdfs:label>
    <rdfs:comment>Specifies a list of External URLs that can be redirected to as part of logging in or logging out of the Windows Web App.</rdfs:comment>
    <rdfs:domain rdf:resource="http://example.org/onto/class/azurerm_linux_function_app"/>
    <rdfs:range rdf:resource="http://www.w3.org/2001/XMLSchema#string"/>
  </owl:DatatypeProperty>
  <owl:DatatypeProperty rdf:about="http://example.org/onto/prop/azurerm_linux_function_app_default_provider">
    <rdfs:label>default_provider</rdfs:label>
    <rdfs:comment>The default authentication provider to use when multiple providers are configured. Possible values include: `AzureActiveDirectory`, `Facebook`, `Google`, `MicrosoftAccount`, `Twitter`, `Github`.</rdfs:comment>
    <rdfs:domain rdf:resource="http://example.org/onto/class/azurerm_linux_function_app"/>
    <rdfs:range rdf:resource="http://www.w3.org/2001/XMLSchema#string"/>
  </owl:DatatypeProperty>
  <owl:DatatypeProperty rdf:about="http://example.org/onto/prop/azurerm_linux_function_app_enabled">
    <rdfs:label>enabled</rdfs:label>
    <rdfs:comment>Should the Authentication / Authorization feature be enabled?</rdfs:comment>
    <rdfs:domain rdf:resource="http://example.org/onto/class/azurerm_linux_function_app"/>
    <rdfs:range rdf:resource="http://www.w3.org/2001/XMLSchema#string"/>
  </owl:DatatypeProperty>
  <owl:DatatypeProperty rdf:about="http://example.org/onto/prop/azurerm_linux_function_app_issuer">
    <rdfs:label>issuer</rdfs:label>
    <rdfs:comment>The OpenID Connect Issuer URI that represents the entity which issues access tokens.</rdfs:comment>
    <rdfs:domain rdf:resource="http://example.org/onto/class/azurerm_linux_function_app"/>
    <rdfs:range rdf:resource="http://www.w3.org/2001/XMLSchema#string"/>
  </owl:DatatypeProperty>
  <owl:DatatypeProperty rdf:about="http://example.org/onto/prop/azurerm_linux_function_app_runtime_version">
    <rdfs:label>runtime_version</rdfs:label>
    <rdfs:comment>The RuntimeVersion of the Authentication / Authorization feature in use.</rdfs:comment>
    <rdfs:domain rdf:resource="http://example.org/onto/class/azurerm_linux_function_app"/>
    <rdfs:range rdf:resource="http://www.w3.org/2001/XMLSchema#string"/>
  </owl:DatatypeProperty>
  <owl:DatatypeProperty rdf:about="http://example.org/onto/prop/azurerm_linux_function_app_token_refresh_extension_hours">
    <rdfs:label>token_refresh_extension_hours</rdfs:label>
    <rdfs:comment>The number of hours after session token expiration that a session token can be used to call the token refresh API. Defaults to `72` hours.</rdfs:comment>
    <rdfs:domain rdf:resource="http://example.org/onto/class/azurerm_linux_function_app"/>
    <rdfs:range rdf:resource="http://www.w3.org/2001/XMLSchema#string"/>
  </owl:DatatypeProperty>
  <owl:DatatypeProperty rdf:about="http://example.org/onto/prop/azurerm_linux_function_app_token_store_enabled">
    <rdfs:label>token_store_enabled</rdfs:label>
    <rdfs:comment>Should the Windows Web App durably store platform-specific security tokens that are obtained during login flows? Defaults to `false`.</rdfs:comment>
    <rdfs:domain rdf:resource="http://example.org/onto/class/azurerm_linux_function_app"/>
    <rdfs:range rdf:resource="http://www.w3.org/2001/XMLSchema#string"/>
  </owl:DatatypeProperty>
  <owl:DatatypeProperty rdf:about="http://example.org/onto/prop/azurerm_linux_function_app_unauthenticated_client_action">
    <rdfs:label>unauthenticated_client_action</rdfs:label>
    <rdfs:comment>The action to take when an unauthenticated client attempts to access the app. Possible values include: `RedirectToLoginPage`, `AllowAnonymous`.</rdfs:comment>
    <rdfs:domain rdf:resource="http://example.org/onto/class/azurerm_linux_function_app"/>
    <rdfs:range rdf:resource="http://www.w3.org/2001/XMLSchema#string"/>
  </owl:DatatypeProperty>
  <owl:DatatypeProperty rdf:about="http://example.org/onto/prop/azurerm_linux_function_app_allowed_audiences">
    <rdfs:label>allowed_audiences</rdfs:label>
    <rdfs:comment>Specifies a list of Allowed audience values to consider when validating JWTs issued by Azure Active Directory.</rdfs:comment>
    <rdfs:domain rdf:resource="http://example.org/onto/class/azurerm_linux_function_app"/>
    <rdfs:range rdf:resource="http://www.w3.org/2001/XMLSchema#string"/>
  </owl:DatatypeProperty>
  <owl:DatatypeProperty rdf:about="http://example.org/onto/prop/azurerm_linux_function_app_client_id">
    <rdfs:label>client_id</rdfs:label>
    <rdfs:comment>The ID of the Client to use to authenticate with Azure Active Directory.</rdfs:comment>
    <rdfs:domain rdf:resource="http://example.org/onto/class/azurerm_linux_function_app"/>
    <rdfs:range rdf:resource="http://www.w3.org/2001/XMLSchema#string"/>
  </owl:DatatypeProperty>
  <owl:DatatypeProperty rdf:about="http://example.org/onto/prop/azurerm_linux_function_app_client_secret">
    <rdfs:label>client_secret</rdfs:label>
    <rdfs:comment>The Client Secret for the Client ID. Cannot be used with `client_secret_setting_name`.</rdfs:comment>
    <rdfs:domain rdf:resource="http://example.org/onto/class/azurerm_linux_function_app"/>
    <rdfs:range rdf:resource="http://www.w3.org/2001/XMLSchema#string"/>
  </owl:DatatypeProperty>
  <owl:DatatypeProperty rdf:about="http://example.org/onto/prop/azurerm_linux_function_app_client_secret_setting_name">
    <rdfs:label>client_secret_setting_name</rdfs:label>
    <rdfs:comment>The App Setting name that contains the client secret of the Client. Cannot be used with `client_secret`.</rdfs:comment>
    <rdfs:domain rdf:resource="http://example.org/onto/class/azurerm_linux_function_app"/>
    <rdfs:range rdf:resource="http://www.w3.org/2001/XMLSchema#string"/>
  </owl:DatatypeProperty>
  <owl:DatatypeProperty rdf:about="http://example.org/onto/prop/azurerm_linux_function_app_app_id">
    <rdfs:label>app_id</rdfs:label>
    <rdfs:comment>The App ID of the Facebook app used for login.</rdfs:comment>
    <rdfs:domain rdf:resource="http://example.org/onto/class/azurerm_linux_function_app"/>
    <rdfs:range rdf:resource="http://www.w3.org/2001/XMLSchema#string"/>
  </owl:DatatypeProperty>
  <owl:DatatypeProperty rdf:about="http://example.org/onto/prop/azurerm_linux_function_app_app_secret">
    <rdfs:label>app_secret</rdfs:label>
    <rdfs:comment>The App Secret of the Facebook app used for Facebook Login. Cannot be specified with `app_secret_setting_name`.</rdfs:comment>
    <rdfs:domain rdf:resource="http://example.org/onto/class/azurerm_linux_function_app"/>
    <rdfs:range rdf:resource="http://www.w3.org/2001/XMLSchema#string"/>
  </owl:DatatypeProperty>
  <owl:DatatypeProperty rdf:about="http://example.org/onto/prop/azurerm_linux_function_app_app_secret_setting_name">
    <rdfs:label>app_secret_setting_name</rdfs:label>
    <rdfs:comment>The app setting name that contains the `app_secret` value used for Facebook Login. Cannot be specified with `app_secret`.</rdfs:comment>
    <rdfs:domain rdf:resource="http://example.org/onto/class/azurerm_linux_function_app"/>
    <rdfs:range rdf:resource="http://www.w3.org/2001/XMLSchema#string"/>
  </owl:DatatypeProperty>
  <owl:DatatypeProperty rdf:about="http://example.org/onto/prop/azurerm_linux_function_app_oauth_scopes">
    <rdfs:label>oauth_scopes</rdfs:label>
    <rdfs:comment>Specifies a list of OAuth 2.0 scopes to be requested as part of Facebook Login authentication.</rdfs:comment>
    <rdfs:domain rdf:resource="http://example.org/onto/class/azurerm_linux_function_app"/>
    <rdfs:range rdf:resource="http://www.w3.org/2001/XMLSchema#string"/>
  </owl:DatatypeProperty>
  <owl:DatatypeProperty rdf:about="http://example.org/onto/prop/azurerm_linux_function_app_client_id">
    <rdfs:label>client_id</rdfs:label>
    <rdfs:comment>The ID of the GitHub app used for login.</rdfs:comment>
    <rdfs:domain rdf:resource="http://example.org/onto/class/azurerm_linux_function_app"/>
    <rdfs:range rdf:resource="http://www.w3.org/2001/XMLSchema#string"/>
  </owl:DatatypeProperty>
  <owl:DatatypeProperty rdf:about="http://example.org/onto/prop/azurerm_linux_function_app_client_secret">
    <rdfs:label>client_secret</rdfs:label>
    <rdfs:comment>The Client Secret of the GitHub app used for GitHub Login. Cannot be specified with `client_secret_setting_name`.</rdfs:comment>
    <rdfs:domain rdf:resource="http://example.org/onto/class/azurerm_linux_function_app"/>
    <rdfs:range rdf:resource="http://www.w3.org/2001/XMLSchema#string"/>
  </owl:DatatypeProperty>
  <owl:DatatypeProperty rdf:about="http://example.org/onto/prop/azurerm_linux_function_app_client_secret_setting_name">
    <rdfs:label>client_secret_setting_name</rdfs:label>
    <rdfs:comment>The app setting name that contains the `client_secret` value used for GitHub Login. Cannot be specified with `client_secret`.</rdfs:comment>
    <rdfs:domain rdf:resource="http://example.org/onto/class/azurerm_linux_function_app"/>
    <rdfs:range rdf:resource="http://www.w3.org/2001/XMLSchema#string"/>
  </owl:DatatypeProperty>
  <owl:DatatypeProperty rdf:about="http://example.org/onto/prop/azurerm_linux_function_app_oauth_scopes">
    <rdfs:label>oauth_scopes</rdfs:label>
    <rdfs:comment>Specifies a list of OAuth 2.0 scopes that will be requested as part of GitHub Login authentication.</rdfs:comment>
    <rdfs:domain rdf:resource="http://example.org/onto/class/azurerm_linux_function_app"/>
    <rdfs:range rdf:resource="http://www.w3.org/2001/XMLSchema#string"/>
  </owl:DatatypeProperty>
  <owl:DatatypeProperty rdf:about="http://example.org/onto/prop/azurerm_linux_function_app_client_id">
    <rdfs:label>client_id</rdfs:label>
    <rdfs:comment>The OpenID Connect Client ID for the Google web application.</rdfs:comment>
    <rdfs:domain rdf:resource="http://example.org/onto/class/azurerm_linux_function_app"/>
    <rdfs:range rdf:resource="http://www.w3.org/2001/XMLSchema#string"/>
  </owl:DatatypeProperty>
  <owl:DatatypeProperty rdf:about="http://example.org/onto/prop/azurerm_linux_function_app_client_secret">
    <rdfs:label>client_secret</rdfs:label>
    <rdfs:comment>The client secret associated with the Google web application.  Cannot be specified with `client_secret_setting_name`.</rdfs:comment>
    <rdfs:domain rdf:resource="http://example.org/onto/class/azurerm_linux_function_app"/>
    <rdfs:range rdf:resource="http://www.w3.org/2001/XMLSchema#string"/>
  </owl:DatatypeProperty>
  <owl:DatatypeProperty rdf:about="http://example.org/onto/prop/azurerm_linux_function_app_client_secret_setting_name">
    <rdfs:label>client_secret_setting_name</rdfs:label>
    <rdfs:comment>The app setting name that contains the `client_secret` value used for Google Login. Cannot be specified with `client_secret`.</rdfs:comment>
    <rdfs:domain rdf:resource="http://example.org/onto/class/azurerm_linux_function_app"/>
    <rdfs:range rdf:resource="http://www.w3.org/2001/XMLSchema#string"/>
  </owl:DatatypeProperty>
  <owl:DatatypeProperty rdf:about="http://example.org/onto/prop/azurerm_linux_function_app_oauth_scopes">
    <rdfs:label>oauth_scopes</rdfs:label>
    <rdfs:comment>Specifies a list of OAuth 2.0 scopes that will be requested as part of Google Sign-In authentication. If not specified, "openid", "profile", and "email" are used as default scopes.</rdfs:comment>
    <rdfs:domain rdf:resource="http://example.org/onto/class/azurerm_linux_function_app"/>
    <rdfs:range rdf:resource="http://www.w3.org/2001/XMLSchema#string"/>
  </owl:DatatypeProperty>
  <owl:DatatypeProperty rdf:about="http://example.org/onto/prop/azurerm_linux_function_app_client_id">
    <rdfs:label>client_id</rdfs:label>
    <rdfs:comment>The OAuth 2.0 client ID that was created for the app used for authentication.</rdfs:comment>
    <rdfs:domain rdf:resource="http://example.org/onto/class/azurerm_linux_function_app"/>
    <rdfs:range rdf:resource="http://www.w3.org/2001/XMLSchema#string"/>
  </owl:DatatypeProperty>
  <owl:DatatypeProperty rdf:about="http://example.org/onto/prop/azurerm_linux_function_app_client_secret">
    <rdfs:label>client_secret</rdfs:label>
    <rdfs:comment>The OAuth 2.0 client secret that was created for the app used for authentication. Cannot be specified with `client_secret_setting_name`.</rdfs:comment>
    <rdfs:domain rdf:resource="http://example.org/onto/class/azurerm_linux_function_app"/>
    <rdfs:range rdf:resource="http://www.w3.org/2001/XMLSchema#string"/>
  </owl:DatatypeProperty>
  <owl:DatatypeProperty rdf:about="http://example.org/onto/prop/azurerm_linux_function_app_client_secret_setting_name">
    <rdfs:label>client_secret_setting_name</rdfs:label>
    <rdfs:comment>The app setting name containing the OAuth 2.0 client secret that was created for the app used for authentication. Cannot be specified with `client_secret`.</rdfs:comment>
    <rdfs:domain rdf:resource="http://example.org/onto/class/azurerm_linux_function_app"/>
    <rdfs:range rdf:resource="http://www.w3.org/2001/XMLSchema#string"/>
  </owl:DatatypeProperty>
  <owl:DatatypeProperty rdf:about="http://example.org/onto/prop/azurerm_linux_function_app_oauth_scopes">
    <rdfs:label>oauth_scopes</rdfs:label>
    <rdfs:comment>The list of OAuth 2.0 scopes that will be requested as part of Microsoft Account authentication. If not specified, `wl.basic` is used as the default scope.</rdfs:comment>
    <rdfs:domain rdf:resource="http://example.org/onto/class/azurerm_linux_function_app"/>
    <rdfs:range rdf:resource="http://www.w3.org/2001/XMLSchema#string"/>
  </owl:DatatypeProperty>
  <owl:DatatypeProperty rdf:about="http://example.org/onto/prop/azurerm_linux_function_app_consumer_key">
    <rdfs:label>consumer_key</rdfs:label>
    <rdfs:comment>The OAuth 1.0a consumer key of the Twitter application used for sign-in.</rdfs:comment>
    <rdfs:domain rdf:resource="http://example.org/onto/class/azurerm_linux_function_app"/>
    <rdfs:range rdf:resource="http://www.w3.org/2001/XMLSchema#string"/>
  </owl:DatatypeProperty>
  <owl:DatatypeProperty rdf:about="http://example.org/onto/prop/azurerm_linux_function_app_consumer_secret">
    <rdfs:label>consumer_secret</rdfs:label>
    <rdfs:comment>The OAuth 1.0a consumer secret of the Twitter application used for sign-in. Cannot be specified with `consumer_secret_setting_name`.</rdfs:comment>
    <rdfs:domain rdf:resource="http://example.org/onto/class/azurerm_linux_function_app"/>
    <rdfs:range rdf:resource="http://www.w3.org/2001/XMLSchema#string"/>
  </owl:DatatypeProperty>
  <owl:DatatypeProperty rdf:about="http://example.org/onto/prop/azurerm_linux_function_app_consumer_secret_setting_name">
    <rdfs:label>consumer_secret_setting_name</rdfs:label>
    <rdfs:comment>The app setting name that contains the OAuth 1.0a consumer secret of the Twitter application used for sign-in. Cannot be specified with `consumer_secret`.</rdfs:comment>
    <rdfs:domain rdf:resource="http://example.org/onto/class/azurerm_linux_function_app"/>
    <rdfs:range rdf:resource="http://www.w3.org/2001/XMLSchema#string"/>
  </owl:DatatypeProperty>
  <owl:DatatypeProperty rdf:about="http://example.org/onto/prop/azurerm_linux_function_app_auth_enabled">
    <rdfs:label>auth_enabled</rdfs:label>
    <rdfs:comment>Should the AuthV2 Settings be enabled. Defaults to `false`</rdfs:comment>
    <rdfs:domain rdf:resource="http://example.org/onto/class/azurerm_linux_function_app"/>
    <rdfs:range rdf:resource="http://www.w3.org/2001/XMLSchema#string"/>
  </owl:DatatypeProperty>
  <owl:DatatypeProperty rdf:about="http://example.org/onto/prop/azurerm_linux_function_app_config_file_path">
    <rdfs:label>config_file_path</rdfs:label>
    <rdfs:comment>The path to the App Auth settings. **Note:** Relative Paths are evaluated from the Site Root directory.</rdfs:comment>
    <rdfs:domain rdf:resource="http://example.org/onto/class/azurerm_linux_function_app"/>
    <rdfs:range rdf:resource="http://www.w3.org/2001/XMLSchema#string"/>
  </owl:DatatypeProperty>
  <owl:DatatypeProperty rdf:about="http://example.org/onto/prop/azurerm_linux_function_app_default_provider">
    <rdfs:label>default_provider</rdfs:label>
    <rdfs:comment>The Default Authentication Provider to use when the `unauthenticated_action` is set to `RedirectToLoginPage`. Possible values include: `apple`, `azureactivedirectory`, `facebook`, `github`, `google`, `twitter` and the `name` of your `custom_oidc_v2` provider.</rdfs:comment>
    <rdfs:domain rdf:resource="http://example.org/onto/class/azurerm_linux_function_app"/>
    <rdfs:range rdf:resource="http://www.w3.org/2001/XMLSchema#string"/>
  </owl:DatatypeProperty>
  <owl:DatatypeProperty rdf:about="http://example.org/onto/prop/azurerm_linux_function_app_excluded_paths">
    <rdfs:label>excluded_paths</rdfs:label>
    <rdfs:comment>The paths which should be excluded from the `unauthenticated_action` when it is set to `RedirectToLoginPage`.</rdfs:comment>
    <rdfs:domain rdf:resource="http://example.org/onto/class/azurerm_linux_function_app"/>
    <rdfs:range rdf:resource="http://www.w3.org/2001/XMLSchema#string"/>
  </owl:DatatypeProperty>
  <owl:DatatypeProperty rdf:about="http://example.org/onto/prop/azurerm_linux_function_app_forward_proxy_convention">
    <rdfs:label>forward_proxy_convention</rdfs:label>
    <rdfs:comment>The convention used to determine the url of the request made. Possible values include `ForwardProxyConventionNoProxy`, `ForwardProxyConventionStandard`, `ForwardProxyConventionCustom`. Defaults to `ForwardProxyConventionNoProxy`</rdfs:comment>
    <rdfs:domain rdf:resource="http://example.org/onto/class/azurerm_linux_function_app"/>
    <rdfs:range rdf:resource="http://www.w3.org/2001/XMLSchema#string"/>
  </owl:DatatypeProperty>
  <owl:DatatypeProperty rdf:about="http://example.org/onto/prop/azurerm_linux_function_app_forward_proxy_custom_host_header_name">
    <rdfs:label>forward_proxy_custom_host_header_name</rdfs:label>
    <rdfs:comment>The name of the header containing the host of the request.</rdfs:comment>
    <rdfs:domain rdf:resource="http://example.org/onto/class/azurerm_linux_function_app"/>
    <rdfs:range rdf:resource="http://www.w3.org/2001/XMLSchema#string"/>
  </owl:DatatypeProperty>
  <owl:DatatypeProperty rdf:about="http://example.org/onto/prop/azurerm_linux_function_app_forward_proxy_custom_scheme_header_name">
    <rdfs:label>forward_proxy_custom_scheme_header_name</rdfs:label>
    <rdfs:comment>The name of the header containing the scheme of the request.</rdfs:comment>
    <rdfs:domain rdf:resource="http://example.org/onto/class/azurerm_linux_function_app"/>
    <rdfs:range rdf:resource="http://www.w3.org/2001/XMLSchema#string"/>
  </owl:DatatypeProperty>
  <owl:DatatypeProperty rdf:about="http://example.org/onto/prop/azurerm_linux_function_app_http_route_api_prefix">
    <rdfs:label>http_route_api_prefix</rdfs:label>
    <rdfs:comment>The prefix that should precede all the authentication and authorisation paths. Defaults to `/.auth`</rdfs:comment>
    <rdfs:domain rdf:resource="http://example.org/onto/class/azurerm_linux_function_app"/>
    <rdfs:range rdf:resource="http://www.w3.org/2001/XMLSchema#string"/>
  </owl:DatatypeProperty>
  <owl:DatatypeProperty rdf:about="http://example.org/onto/prop/azurerm_linux_function_app_require_authentication">
    <rdfs:label>require_authentication</rdfs:label>
    <rdfs:comment>Should the authentication flow be used for all requests.</rdfs:comment>
    <rdfs:domain rdf:resource="http://example.org/onto/class/azurerm_linux_function_app"/>
    <rdfs:range rdf:resource="http://www.w3.org/2001/XMLSchema#string"/>
  </owl:DatatypeProperty>
  <owl:DatatypeProperty rdf:about="http://example.org/onto/prop/azurerm_linux_function_app_require_https">
    <rdfs:label>require_https</rdfs:label>
    <rdfs:comment>Should HTTPS be required on connections? Defaults to true.</rdfs:comment>
    <rdfs:domain rdf:resource="http://example.org/onto/class/azurerm_linux_function_app"/>
    <rdfs:range rdf:resource="http://www.w3.org/2001/XMLSchema#string"/>
  </owl:DatatypeProperty>
  <owl:DatatypeProperty rdf:about="http://example.org/onto/prop/azurerm_linux_function_app_runtime_version">
    <rdfs:label>runtime_version</rdfs:label>
    <rdfs:comment>The Runtime Version of the Authentication and Authorisation feature of this App. Defaults to `~1`</rdfs:comment>
    <rdfs:domain rdf:resource="http://example.org/onto/class/azurerm_linux_function_app"/>
    <rdfs:range rdf:resource="http://www.w3.org/2001/XMLSchema#string"/>
  </owl:DatatypeProperty>
  <owl:DatatypeProperty rdf:about="http://example.org/onto/prop/azurerm_linux_function_app_unauthenticated_action">
    <rdfs:label>unauthenticated_action</rdfs:label>
    <rdfs:comment>The action to take for requests made without authentication. Possible values include `RedirectToLoginPage`, `AllowAnonymous`, `Return401`, and `Return403`. Defaults to `RedirectToLoginPage`.</rdfs:comment>
    <rdfs:domain rdf:resource="http://example.org/onto/class/azurerm_linux_function_app"/>
    <rdfs:range rdf:resource="http://www.w3.org/2001/XMLSchema#string"/>
  </owl:DatatypeProperty>
  <owl:DatatypeProperty rdf:about="http://example.org/onto/prop/azurerm_linux_function_app_allowed_applications">
    <rdfs:label>allowed_applications</rdfs:label>
    <rdfs:comment>The list of allowed Applications for the Default Authorisation Policy.</rdfs:comment>
    <rdfs:domain rdf:resource="http://example.org/onto/class/azurerm_linux_function_app"/>
    <rdfs:range rdf:resource="http://www.w3.org/2001/XMLSchema#string"/>
  </owl:DatatypeProperty>
  <owl:DatatypeProperty rdf:about="http://example.org/onto/prop/azurerm_linux_function_app_allowed_audiences">
    <rdfs:label>allowed_audiences</rdfs:label>
    <rdfs:comment>Specifies a list of Allowed audience values to consider when validating JWTs issued by Azure Active Directory.</rdfs:comment>
    <rdfs:domain rdf:resource="http://example.org/onto/class/azurerm_linux_function_app"/>
    <rdfs:range rdf:resource="http://www.w3.org/2001/XMLSchema#string"/>
  </owl:DatatypeProperty>
  <owl:DatatypeProperty rdf:about="http://example.org/onto/prop/azurerm_linux_function_app_allowed_groups">
    <rdfs:label>allowed_groups</rdfs:label>
    <rdfs:comment>The list of allowed Group Names for the Default Authorisation Policy.</rdfs:comment>
    <rdfs:domain rdf:resource="http://example.org/onto/class/azurerm_linux_function_app"/>
    <rdfs:range rdf:resource="http://www.w3.org/2001/XMLSchema#string"/>
  </owl:DatatypeProperty>
  <owl:DatatypeProperty rdf:about="http://example.org/onto/prop/azurerm_linux_function_app_allowed_identities">
    <rdfs:label>allowed_identities</rdfs:label>
    <rdfs:comment>The list of allowed Identities for the Default Authorisation Policy.</rdfs:comment>
    <rdfs:domain rdf:resource="http://example.org/onto/class/azurerm_linux_function_app"/>
    <rdfs:range rdf:resource="http://www.w3.org/2001/XMLSchema#string"/>
  </owl:DatatypeProperty>
  <owl:DatatypeProperty rdf:about="http://example.org/onto/prop/azurerm_linux_function_app_client_id">
    <rdfs:label>client_id</rdfs:label>
    <rdfs:comment>The ID of the Client to use to authenticate with Azure Active Directory.</rdfs:comment>
    <rdfs:domain rdf:resource="http://example.org/onto/class/azurerm_linux_function_app"/>
    <rdfs:range rdf:resource="http://www.w3.org/2001/XMLSchema#string"/>
  </owl:DatatypeProperty>
  <owl:DatatypeProperty rdf:about="http://example.org/onto/prop/azurerm_linux_function_app_client_secret_certificate_thumbprint">
    <rdfs:label>client_secret_certificate_thumbprint</rdfs:label>
    <rdfs:comment>The thumbprint of the certificate used for signing purposes.</rdfs:comment>
    <rdfs:domain rdf:resource="http://example.org/onto/class/azurerm_linux_function_app"/>
    <rdfs:range rdf:resource="http://www.w3.org/2001/XMLSchema#string"/>
  </owl:DatatypeProperty>
  <owl:DatatypeProperty rdf:about="http://example.org/onto/prop/azurerm_linux_function_app_client_secret_setting_name">
    <rdfs:label>client_secret_setting_name</rdfs:label>
    <rdfs:comment>The App Setting name that contains the client secret of the Client.</rdfs:comment>
    <rdfs:domain rdf:resource="http://example.org/onto/class/azurerm_linux_function_app"/>
    <rdfs:range rdf:resource="http://www.w3.org/2001/XMLSchema#string"/>
  </owl:DatatypeProperty>
  <owl:DatatypeProperty rdf:about="http://example.org/onto/prop/azurerm_linux_function_app_jwt_allowed_client_applications">
    <rdfs:label>jwt_allowed_client_applications</rdfs:label>
    <rdfs:comment>A list of Allowed Client Applications in the JWT Claim.</rdfs:comment>
    <rdfs:domain rdf:resource="http://example.org/onto/class/azurerm_linux_function_app"/>
    <rdfs:range rdf:resource="http://www.w3.org/2001/XMLSchema#string"/>
  </owl:DatatypeProperty>
  <owl:DatatypeProperty rdf:about="http://example.org/onto/prop/azurerm_linux_function_app_jwt_allowed_groups">
    <rdfs:label>jwt_allowed_groups</rdfs:label>
    <rdfs:comment>A list of Allowed Groups in the JWT Claim.</rdfs:comment>
    <rdfs:domain rdf:resource="http://example.org/onto/class/azurerm_linux_function_app"/>
    <rdfs:range rdf:resource="http://www.w3.org/2001/XMLSchema#string"/>
  </owl:DatatypeProperty>
  <owl:DatatypeProperty rdf:about="http://example.org/onto/prop/azurerm_linux_function_app_login_parameters">
    <rdfs:label>login_parameters</rdfs:label>
    <rdfs:comment>A map of key-value pairs to send to the Authorisation Endpoint when a user logs in.</rdfs:comment>
    <rdfs:domain rdf:resource="http://example.org/onto/class/azurerm_linux_function_app"/>
    <rdfs:range rdf:resource="http://www.w3.org/2001/XMLSchema#string"/>
  </owl:DatatypeProperty>
  <owl:DatatypeProperty rdf:about="http://example.org/onto/prop/azurerm_linux_function_app_tenant_auth_endpoint">
    <rdfs:label>tenant_auth_endpoint</rdfs:label>
    <rdfs:comment>The Azure Tenant Endpoint for the Authenticating Tenant. e.g. `https://login.microsoftonline.com/v2.0/{tenant-guid}/`.</rdfs:comment>
    <rdfs:domain rdf:resource="http://example.org/onto/class/azurerm_linux_function_app"/>
    <rdfs:range rdf:resource="http://www.w3.org/2001/XMLSchema#string"/>
  </owl:DatatypeProperty>
  <owl:DatatypeProperty rdf:about="http://example.org/onto/prop/azurerm_linux_function_app_www_authentication_disabled">
    <rdfs:label>www_authentication_disabled</rdfs:label>
    <rdfs:comment>Should the www-authenticate provider should be omitted from the request? Defaults to `false`</rdfs:comment>
    <rdfs:domain rdf:resource="http://example.org/onto/class/azurerm_linux_function_app"/>
    <rdfs:range rdf:resource="http://www.w3.org/2001/XMLSchema#string"/>
  </owl:DatatypeProperty>
  <owl:DatatypeProperty rdf:about="http://example.org/onto/prop/azurerm_linux_function_app_client_id">
    <rdfs:label>client_id</rdfs:label>
    <rdfs:comment>The OpenID Connect Client ID for the Apple web application.</rdfs:comment>
    <rdfs:domain rdf:resource="http://example.org/onto/class/azurerm_linux_function_app"/>
    <rdfs:range rdf:resource="http://www.w3.org/2001/XMLSchema#string"/>
  </owl:DatatypeProperty>
  <owl:DatatypeProperty rdf:about="http://example.org/onto/prop/azurerm_linux_function_app_client_secret_setting_name">
    <rdfs:label>client_secret_setting_name</rdfs:label>
    <rdfs:comment>The app setting name that contains the `client_secret` value used for Apple Login.</rdfs:comment>
    <rdfs:domain rdf:resource="http://example.org/onto/class/azurerm_linux_function_app"/>
    <rdfs:range rdf:resource="http://www.w3.org/2001/XMLSchema#string"/>
  </owl:DatatypeProperty>
  <owl:DatatypeProperty rdf:about="http://example.org/onto/prop/azurerm_linux_function_app_login_scopes">
    <rdfs:label>login_scopes</rdfs:label>
    <rdfs:domain rdf:resource="http://example.org/onto/class/azurerm_linux_function_app"/>
    <rdfs:range rdf:resource="http://www.w3.org/2001/XMLSchema#string"/>
  </owl:DatatypeProperty>
  <owl:DatatypeProperty rdf:about="http://example.org/onto/prop/azurerm_linux_function_app_client_id">
    <rdfs:label>client_id</rdfs:label>
    <rdfs:comment>The ID of the Client to use to authenticate with Azure Static Web App Authentication.</rdfs:comment>
    <rdfs:domain rdf:resource="http://example.org/onto/class/azurerm_linux_function_app"/>
    <rdfs:range rdf:resource="http://www.w3.org/2001/XMLSchema#string"/>
  </owl:DatatypeProperty>
  <owl:DatatypeProperty rdf:about="http://example.org/onto/prop/azurerm_linux_function_app_authorisation_endpoint">
    <rdfs:label>authorisation_endpoint</rdfs:label>
    <rdfs:comment>The endpoint to make the Authorisation Request.</rdfs:comment>
    <rdfs:domain rdf:resource="http://example.org/onto/class/azurerm_linux_function_app"/>
    <rdfs:range rdf:resource="http://www.w3.org/2001/XMLSchema#string"/>
  </owl:DatatypeProperty>
  <owl:DatatypeProperty rdf:about="http://example.org/onto/prop/azurerm_linux_function_app_certification_uri">
    <rdfs:label>certification_uri</rdfs:label>
    <rdfs:comment>The endpoint that provides the keys necessary to validate the token.</rdfs:comment>
    <rdfs:domain rdf:resource="http://example.org/onto/class/azurerm_linux_function_app"/>
    <rdfs:range rdf:resource="http://www.w3.org/2001/XMLSchema#string"/>
  </owl:DatatypeProperty>
  <owl:DatatypeProperty rdf:about="http://example.org/onto/prop/azurerm_linux_function_app_client_credential_method">
    <rdfs:label>client_credential_method</rdfs:label>
    <rdfs:comment>The Client Credential Method used. Currently the only supported value is `ClientSecretPost`.</rdfs:comment>
    <rdfs:domain rdf:resource="http://example.org/onto/class/azurerm_linux_function_app"/>
    <rdfs:range rdf:resource="http://www.w3.org/2001/XMLSchema#string"/>
  </owl:DatatypeProperty>
  <owl:DatatypeProperty rdf:about="http://example.org/onto/prop/azurerm_linux_function_app_client_id">
    <rdfs:label>client_id</rdfs:label>
    <rdfs:comment>The ID of the Client to use to authenticate with this Custom OIDC.</rdfs:comment>
    <rdfs:domain rdf:resource="http://example.org/onto/class/azurerm_linux_function_app"/>
    <rdfs:range rdf:resource="http://www.w3.org/2001/XMLSchema#string"/>
  </owl:DatatypeProperty>
  <owl:DatatypeProperty rdf:about="http://example.org/onto/prop/azurerm_linux_function_app_client_secret_setting_name">
    <rdfs:label>client_secret_setting_name</rdfs:label>
    <rdfs:comment>The App Setting name that contains the secret for this Custom OIDC Client.</rdfs:comment>
    <rdfs:domain rdf:resource="http://example.org/onto/class/azurerm_linux_function_app"/>
    <rdfs:range rdf:resource="http://www.w3.org/2001/XMLSchema#string"/>
  </owl:DatatypeProperty>
  <owl:DatatypeProperty rdf:about="http://example.org/onto/prop/azurerm_linux_function_app_issuer_endpoint">
    <rdfs:label>issuer_endpoint</rdfs:label>
    <rdfs:comment>The endpoint that issued the Token.</rdfs:comment>
    <rdfs:domain rdf:resource="http://example.org/onto/class/azurerm_linux_function_app"/>
    <rdfs:range rdf:resource="http://www.w3.org/2001/XMLSchema#string"/>
  </owl:DatatypeProperty>
  <owl:DatatypeProperty rdf:about="http://example.org/onto/prop/azurerm_linux_function_app_name">
    <rdfs:label>name</rdfs:label>
    <rdfs:comment>The name of the Custom OIDC Authentication Provider.</rdfs:comment>
    <rdfs:domain rdf:resource="http://example.org/onto/class/azurerm_linux_function_app"/>
    <rdfs:range rdf:resource="http://www.w3.org/2001/XMLSchema#string"/>
  </owl:DatatypeProperty>
  <owl:DatatypeProperty rdf:about="http://example.org/onto/prop/azurerm_linux_function_app_name_claim_type">
    <rdfs:label>name_claim_type</rdfs:label>
    <rdfs:comment>The name of the claim that contains the users name.</rdfs:comment>
    <rdfs:domain rdf:resource="http://example.org/onto/class/azurerm_linux_function_app"/>
    <rdfs:range rdf:resource="http://www.w3.org/2001/XMLSchema#string"/>
  </owl:DatatypeProperty>
  <owl:DatatypeProperty rdf:about="http://example.org/onto/prop/azurerm_linux_function_app_openid_configuration_endpoint">
    <rdfs:label>openid_configuration_endpoint</rdfs:label>
    <rdfs:comment>The endpoint that contains all the configuration endpoints for this Custom OIDC provider.</rdfs:comment>
    <rdfs:domain rdf:resource="http://example.org/onto/class/azurerm_linux_function_app"/>
    <rdfs:range rdf:resource="http://www.w3.org/2001/XMLSchema#string"/>
  </owl:DatatypeProperty>
  <owl:DatatypeProperty rdf:about="http://example.org/onto/prop/azurerm_linux_function_app_scopes">
    <rdfs:label>scopes</rdfs:label>
    <rdfs:comment>The list of the scopes that should be requested while authenticating.</rdfs:comment>
    <rdfs:domain rdf:resource="http://example.org/onto/class/azurerm_linux_function_app"/>
    <rdfs:range rdf:resource="http://www.w3.org/2001/XMLSchema#string"/>
  </owl:DatatypeProperty>
  <owl:DatatypeProperty rdf:about="http://example.org/onto/prop/azurerm_linux_function_app_token_endpoint">
    <rdfs:label>token_endpoint</rdfs:label>
    <rdfs:comment>The endpoint used to request a Token.</rdfs:comment>
    <rdfs:domain rdf:resource="http://example.org/onto/class/azurerm_linux_function_app"/>
    <rdfs:range rdf:resource="http://www.w3.org/2001/XMLSchema#string"/>
  </owl:DatatypeProperty>
  <owl:DatatypeProperty rdf:about="http://example.org/onto/prop/azurerm_linux_function_app_app_id">
    <rdfs:label>app_id</rdfs:label>
    <rdfs:comment>The App ID of the Facebook app used for login.</rdfs:comment>
    <rdfs:domain rdf:resource="http://example.org/onto/class/azurerm_linux_function_app"/>
    <rdfs:range rdf:resource="http://www.w3.org/2001/XMLSchema#string"/>
  </owl:DatatypeProperty>
  <owl:DatatypeProperty rdf:about="http://example.org/onto/prop/azurerm_linux_function_app_app_secret_setting_name">
    <rdfs:label>app_secret_setting_name</rdfs:label>
    <rdfs:comment>The app setting name that contains the `app_secret` value used for Facebook Login.</rdfs:comment>
    <rdfs:domain rdf:resource="http://example.org/onto/class/azurerm_linux_function_app"/>
    <rdfs:range rdf:resource="http://www.w3.org/2001/XMLSchema#string"/>
  </owl:DatatypeProperty>
  <owl:DatatypeProperty rdf:about="http://example.org/onto/prop/azurerm_linux_function_app_graph_api_version">
    <rdfs:label>graph_api_version</rdfs:label>
    <rdfs:comment>The version of the Facebook API to be used while logging in.</rdfs:comment>
    <rdfs:domain rdf:resource="http://example.org/onto/class/azurerm_linux_function_app"/>
    <rdfs:range rdf:resource="http://www.w3.org/2001/XMLSchema#string"/>
  </owl:DatatypeProperty>
  <owl:DatatypeProperty rdf:about="http://example.org/onto/prop/azurerm_linux_function_app_login_scopes">
    <rdfs:label>login_scopes</rdfs:label>
    <rdfs:comment>Specifies a list of scopes to be requested as part of Facebook Login authentication.</rdfs:comment>
    <rdfs:domain rdf:resource="http://example.org/onto/class/azurerm_linux_function_app"/>
    <rdfs:range rdf:resource="http://www.w3.org/2001/XMLSchema#string"/>
  </owl:DatatypeProperty>
  <owl:DatatypeProperty rdf:about="http://example.org/onto/prop/azurerm_linux_function_app_client_id">
    <rdfs:label>client_id</rdfs:label>
    <rdfs:comment>The ID of the GitHub app used for login.</rdfs:comment>
    <rdfs:domain rdf:resource="http://example.org/onto/class/azurerm_linux_function_app"/>
    <rdfs:range rdf:resource="http://www.w3.org/2001/XMLSchema#string"/>
  </owl:DatatypeProperty>
  <owl:DatatypeProperty rdf:about="http://example.org/onto/prop/azurerm_linux_function_app_client_secret_setting_name">
    <rdfs:label>client_secret_setting_name</rdfs:label>
    <rdfs:comment>The app setting name that contains the `client_secret` value used for GitHub Login.</rdfs:comment>
    <rdfs:domain rdf:resource="http://example.org/onto/class/azurerm_linux_function_app"/>
    <rdfs:range rdf:resource="http://www.w3.org/2001/XMLSchema#string"/>
  </owl:DatatypeProperty>
  <owl:DatatypeProperty rdf:about="http://example.org/onto/prop/azurerm_linux_function_app_login_scopes">
    <rdfs:label>login_scopes</rdfs:label>
    <rdfs:comment>Specifies a list of OAuth 2.0 scopes that will be requested as part of GitHub Login authentication.</rdfs:comment>
    <rdfs:domain rdf:resource="http://example.org/onto/class/azurerm_linux_function_app"/>
    <rdfs:range rdf:resource="http://www.w3.org/2001/XMLSchema#string"/>
  </owl:DatatypeProperty>
  <owl:DatatypeProperty rdf:about="http://example.org/onto/prop/azurerm_linux_function_app_allowed_audiences">
    <rdfs:label>allowed_audiences</rdfs:label>
    <rdfs:comment>Specifies a list of Allowed Audiences that will be requested as part of Google Sign-In authentication.</rdfs:comment>
    <rdfs:domain rdf:resource="http://example.org/onto/class/azurerm_linux_function_app"/>
    <rdfs:range rdf:resource="http://www.w3.org/2001/XMLSchema#string"/>
  </owl:DatatypeProperty>
  <owl:DatatypeProperty rdf:about="http://example.org/onto/prop/azurerm_linux_function_app_client_id">
    <rdfs:label>client_id</rdfs:label>
    <rdfs:comment>The OpenID Connect Client ID for the Google web application.</rdfs:comment>
    <rdfs:domain rdf:resource="http://example.org/onto/class/azurerm_linux_function_app"/>
    <rdfs:range rdf:resource="http://www.w3.org/2001/XMLSchema#string"/>
  </owl:DatatypeProperty>
  <owl:DatatypeProperty rdf:about="http://example.org/onto/prop/azurerm_linux_function_app_client_secret_setting_name">
    <rdfs:label>client_secret_setting_name</rdfs:label>
    <rdfs:comment>The app setting name that contains the `client_secret` value used for Google Login.</rdfs:comment>
    <rdfs:domain rdf:resource="http://example.org/onto/class/azurerm_linux_function_app"/>
    <rdfs:range rdf:resource="http://www.w3.org/2001/XMLSchema#string"/>
  </owl:DatatypeProperty>
  <owl:DatatypeProperty rdf:about="http://example.org/onto/prop/azurerm_linux_function_app_login_scopes">
    <rdfs:label>login_scopes</rdfs:label>
    <rdfs:comment>Specifies a list of Login scopes that will be requested as part of Google Sign-In authentication.</rdfs:comment>
    <rdfs:domain rdf:resource="http://example.org/onto/class/azurerm_linux_function_app"/>
    <rdfs:range rdf:resource="http://www.w3.org/2001/XMLSchema#string"/>
  </owl:DatatypeProperty>
  <owl:DatatypeProperty rdf:about="http://example.org/onto/prop/azurerm_linux_function_app_allowed_external_redirect_urls">
    <rdfs:label>allowed_external_redirect_urls</rdfs:label>
    <rdfs:comment>External URLs that can be redirected to as part of logging in or logging out of the app. This is an advanced setting typically only needed by Windows Store application backends. **Note:** URLs within the current domain are always implicitly allowed.</rdfs:comment>
    <rdfs:domain rdf:resource="http://example.org/onto/class/azurerm_linux_function_app"/>
    <rdfs:range rdf:resource="http://www.w3.org/2001/XMLSchema#string"/>
  </owl:DatatypeProperty>
  <owl:DatatypeProperty rdf:about="http://example.org/onto/prop/azurerm_linux_function_app_cookie_expiration_convention">
    <rdfs:label>cookie_expiration_convention</rdfs:label>
    <rdfs:comment>The method by which cookies expire. Possible values include: `FixedTime`, and `IdentityProviderDerived`. Defaults to `FixedTime`.</rdfs:comment>
    <rdfs:domain rdf:resource="http://example.org/onto/class/azurerm_linux_function_app"/>
    <rdfs:range rdf:resource="http://www.w3.org/2001/XMLSchema#string"/>
  </owl:DatatypeProperty>
  <owl:DatatypeProperty rdf:about="http://example.org/onto/prop/azurerm_linux_function_app_cookie_expiration_time">
    <rdfs:label>cookie_expiration_time</rdfs:label>
    <rdfs:comment>The time after the request is made when the session cookie should expire. Defaults to `08:00:00`.</rdfs:comment>
    <rdfs:domain rdf:resource="http://example.org/onto/class/azurerm_linux_function_app"/>
    <rdfs:range rdf:resource="http://www.w3.org/2001/XMLSchema#string"/>
  </owl:DatatypeProperty>
  <owl:DatatypeProperty rdf:about="http://example.org/onto/prop/azurerm_linux_function_app_logout_endpoint">
    <rdfs:label>logout_endpoint</rdfs:label>
    <rdfs:comment>The endpoint to which logout requests should be made.</rdfs:comment>
    <rdfs:domain rdf:resource="http://example.org/onto/class/azurerm_linux_function_app"/>
    <rdfs:range rdf:resource="http://www.w3.org/2001/XMLSchema#string"/>
  </owl:DatatypeProperty>
  <owl:DatatypeProperty rdf:about="http://example.org/onto/prop/azurerm_linux_function_app_nonce_expiration_time">
    <rdfs:label>nonce_expiration_time</rdfs:label>
    <rdfs:comment>The time after the request is made when the nonce should expire. Defaults to `00:05:00`.</rdfs:comment>
    <rdfs:domain rdf:resource="http://example.org/onto/class/azurerm_linux_function_app"/>
    <rdfs:range rdf:resource="http://www.w3.org/2001/XMLSchema#string"/>
  </owl:DatatypeProperty>
  <owl:DatatypeProperty rdf:about="http://example.org/onto/prop/azurerm_linux_function_app_preserve_url_fragments_for_logins">
    <rdfs:label>preserve_url_fragments_for_logins</rdfs:label>
    <rdfs:comment>Should the fragments from the request be preserved after the login request is made. Defaults to `false`.</rdfs:comment>
    <rdfs:domain rdf:resource="http://example.org/onto/class/azurerm_linux_function_app"/>
    <rdfs:range rdf:resource="http://www.w3.org/2001/XMLSchema#string"/>
  </owl:DatatypeProperty>
  <owl:DatatypeProperty rdf:about="http://example.org/onto/prop/azurerm_linux_function_app_token_refresh_extension_time">
    <rdfs:label>token_refresh_extension_time</rdfs:label>
    <rdfs:comment>The number of hours after session token expiration that a session token can be used to call the token refresh API. Defaults to `72` hours.</rdfs:comment>
    <rdfs:domain rdf:resource="http://example.org/onto/class/azurerm_linux_function_app"/>
    <rdfs:range rdf:resource="http://www.w3.org/2001/XMLSchema#string"/>
  </owl:DatatypeProperty>
  <owl:DatatypeProperty rdf:about="http://example.org/onto/prop/azurerm_linux_function_app_token_store_enabled">
    <rdfs:label>token_store_enabled</rdfs:label>
    <rdfs:comment>Should the Token Store configuration Enabled. Defaults to `false`</rdfs:comment>
    <rdfs:domain rdf:resource="http://example.org/onto/class/azurerm_linux_function_app"/>
    <rdfs:range rdf:resource="http://www.w3.org/2001/XMLSchema#string"/>
  </owl:DatatypeProperty>
  <owl:DatatypeProperty rdf:about="http://example.org/onto/prop/azurerm_linux_function_app_token_store_path">
    <rdfs:label>token_store_path</rdfs:label>
    <rdfs:comment>The directory path in the App Filesystem in which the tokens will be stored.</rdfs:comment>
    <rdfs:domain rdf:resource="http://example.org/onto/class/azurerm_linux_function_app"/>
    <rdfs:range rdf:resource="http://www.w3.org/2001/XMLSchema#string"/>
  </owl:DatatypeProperty>
  <owl:DatatypeProperty rdf:about="http://example.org/onto/prop/azurerm_linux_function_app_token_store_sas_setting_name">
    <rdfs:label>token_store_sas_setting_name</rdfs:label>
    <rdfs:comment>The name of the app setting which contains the SAS URL of the blob storage containing the tokens.</rdfs:comment>
    <rdfs:domain rdf:resource="http://example.org/onto/class/azurerm_linux_function_app"/>
    <rdfs:range rdf:resource="http://www.w3.org/2001/XMLSchema#string"/>
  </owl:DatatypeProperty>
  <owl:DatatypeProperty rdf:about="http://example.org/onto/prop/azurerm_linux_function_app_validate_nonce">
    <rdfs:label>validate_nonce</rdfs:label>
    <rdfs:comment>Should the nonce be validated while completing the login flow. Defaults to `true`.</rdfs:comment>
    <rdfs:domain rdf:resource="http://example.org/onto/class/azurerm_linux_function_app"/>
    <rdfs:range rdf:resource="http://www.w3.org/2001/XMLSchema#string"/>
  </owl:DatatypeProperty>
  <owl:DatatypeProperty rdf:about="http://example.org/onto/prop/azurerm_linux_function_app_allowed_audiences">
    <rdfs:label>allowed_audiences</rdfs:label>
    <rdfs:comment>Specifies a list of Allowed Audiences that will be requested as part of Microsoft Sign-In authentication.</rdfs:comment>
    <rdfs:domain rdf:resource="http://example.org/onto/class/azurerm_linux_function_app"/>
    <rdfs:range rdf:resource="http://www.w3.org/2001/XMLSchema#string"/>
  </owl:DatatypeProperty>
  <owl:DatatypeProperty rdf:about="http://example.org/onto/prop/azurerm_linux_function_app_client_id">
    <rdfs:label>client_id</rdfs:label>
    <rdfs:comment>The OAuth 2.0 client ID that was created for the app used for authentication.</rdfs:comment>
    <rdfs:domain rdf:resource="http://example.org/onto/class/azurerm_linux_function_app"/>
    <rdfs:range rdf:resource="http://www.w3.org/2001/XMLSchema#string"/>
  </owl:DatatypeProperty>
  <owl:DatatypeProperty rdf:about="http://example.org/onto/prop/azurerm_linux_function_app_client_secret_setting_name">
    <rdfs:label>client_secret_setting_name</rdfs:label>
    <rdfs:comment>The app setting name containing the OAuth 2.0 client secret that was created for the app used for authentication.</rdfs:comment>
    <rdfs:domain rdf:resource="http://example.org/onto/class/azurerm_linux_function_app"/>
    <rdfs:range rdf:resource="http://www.w3.org/2001/XMLSchema#string"/>
  </owl:DatatypeProperty>
  <owl:DatatypeProperty rdf:about="http://example.org/onto/prop/azurerm_linux_function_app_login_scopes">
    <rdfs:label>login_scopes</rdfs:label>
    <rdfs:comment>The list of Login scopes that will be requested as part of Microsoft Account authentication.</rdfs:comment>
    <rdfs:domain rdf:resource="http://example.org/onto/class/azurerm_linux_function_app"/>
    <rdfs:range rdf:resource="http://www.w3.org/2001/XMLSchema#string"/>
  </owl:DatatypeProperty>
  <owl:DatatypeProperty rdf:about="http://example.org/onto/prop/azurerm_linux_function_app_consumer_key">
    <rdfs:label>consumer_key</rdfs:label>
    <rdfs:comment>The OAuth 1.0a consumer key of the Twitter application used for sign-in.</rdfs:comment>
    <rdfs:domain rdf:resource="http://example.org/onto/class/azurerm_linux_function_app"/>
    <rdfs:range rdf:resource="http://www.w3.org/2001/XMLSchema#string"/>
  </owl:DatatypeProperty>
  <owl:DatatypeProperty rdf:about="http://example.org/onto/prop/azurerm_linux_function_app_consumer_secret_setting_name">
    <rdfs:label>consumer_secret_setting_name</rdfs:label>
    <rdfs:comment>The app setting name that contains the OAuth 1.0a consumer secret of the Twitter application used for sign-in.</rdfs:comment>
    <rdfs:domain rdf:resource="http://example.org/onto/class/azurerm_linux_function_app"/>
    <rdfs:range rdf:resource="http://www.w3.org/2001/XMLSchema#string"/>
  </owl:DatatypeProperty>
  <owl:DatatypeProperty rdf:about="http://example.org/onto/prop/azurerm_linux_function_app_enabled">
    <rdfs:label>enabled</rdfs:label>
    <rdfs:comment>Should this backup job be enabled?</rdfs:comment>
    <rdfs:domain rdf:resource="http://example.org/onto/class/azurerm_linux_function_app"/>
    <rdfs:range rdf:resource="http://www.w3.org/2001/XMLSchema#string"/>
  </owl:DatatypeProperty>
  <owl:DatatypeProperty rdf:about="http://example.org/onto/prop/azurerm_linux_function_app_name">
    <rdfs:label>name</rdfs:label>
    <rdfs:comment>The name which should be used for this Backup.</rdfs:comment>
    <rdfs:domain rdf:resource="http://example.org/onto/class/azurerm_linux_function_app"/>
    <rdfs:range rdf:resource="http://www.w3.org/2001/XMLSchema#string"/>
  </owl:DatatypeProperty>
  <owl:DatatypeProperty rdf:about="http://example.org/onto/prop/azurerm_linux_function_app_storage_account_url">
    <rdfs:label>storage_account_url</rdfs:label>
    <rdfs:comment>The SAS URL to the container.</rdfs:comment>
    <rdfs:domain rdf:resource="http://example.org/onto/class/azurerm_linux_function_app"/>
    <rdfs:range rdf:resource="http://www.w3.org/2001/XMLSchema#string"/>
  </owl:DatatypeProperty>
  <owl:DatatypeProperty rdf:about="http://example.org/onto/prop/azurerm_linux_function_app_frequency_interval">
    <rdfs:label>frequency_interval</rdfs:label>
    <rdfs:comment>How often the backup should be executed (e.g. for weekly backup, this should be set to `7` and `frequency_unit` should be set to `Day`).</rdfs:comment>
    <rdfs:domain rdf:resource="http://example.org/onto/class/azurerm_linux_function_app"/>
    <rdfs:range rdf:resource="http://www.w3.org/2001/XMLSchema#string"/>
  </owl:DatatypeProperty>
  <owl:DatatypeProperty rdf:about="http://example.org/onto/prop/azurerm_linux_function_app_frequency_unit">
    <rdfs:label>frequency_unit</rdfs:label>
    <rdfs:comment>The unit of time for how often the backup should take place. Possible values include: `Day` and `Hour`.</rdfs:comment>
    <rdfs:domain rdf:resource="http://example.org/onto/class/azurerm_linux_function_app"/>
    <rdfs:range rdf:resource="http://www.w3.org/2001/XMLSchema#string"/>
  </owl:DatatypeProperty>
  <owl:DatatypeProperty rdf:about="http://example.org/onto/prop/azurerm_linux_function_app_keep_at_least_one_backup">
    <rdfs:label>keep_at_least_one_backup</rdfs:label>
    <rdfs:comment>Should the service keep at least one backup, regardless of age of backup. Defaults to `false`.</rdfs:comment>
    <rdfs:domain rdf:resource="http://example.org/onto/class/azurerm_linux_function_app"/>
    <rdfs:range rdf:resource="http://www.w3.org/2001/XMLSchema#string"/>
  </owl:DatatypeProperty>
  <owl:DatatypeProperty rdf:about="http://example.org/onto/prop/azurerm_linux_function_app_last_execution_time">
    <rdfs:label>last_execution_time</rdfs:label>
    <rdfs:comment>The time the backup was last attempted.</rdfs:comment>
    <rdfs:domain rdf:resource="http://example.org/onto/class/azurerm_linux_function_app"/>
    <rdfs:range rdf:resource="http://www.w3.org/2001/XMLSchema#string"/>
  </owl:DatatypeProperty>
  <owl:DatatypeProperty rdf:about="http://example.org/onto/prop/azurerm_linux_function_app_retention_period_days">
    <rdfs:label>retention_period_days</rdfs:label>
    <rdfs:comment>After how many days backups should be deleted.</rdfs:comment>
    <rdfs:domain rdf:resource="http://example.org/onto/class/azurerm_linux_function_app"/>
    <rdfs:range rdf:resource="http://www.w3.org/2001/XMLSchema#string"/>
  </owl:DatatypeProperty>
  <owl:DatatypeProperty rdf:about="http://example.org/onto/prop/azurerm_linux_function_app_start_time">
    <rdfs:label>start_time</rdfs:label>
    <rdfs:comment>When the schedule should start working in RFC-3339 format.</rdfs:comment>
    <rdfs:domain rdf:resource="http://example.org/onto/class/azurerm_linux_function_app"/>
    <rdfs:range rdf:resource="http://www.w3.org/2001/XMLSchema#string"/>
  </owl:DatatypeProperty>
  <owl:DatatypeProperty rdf:about="http://example.org/onto/prop/azurerm_linux_function_app_name">
    <rdfs:label>name</rdfs:label>
    <rdfs:comment>The name which should be used for this Connection.</rdfs:comment>
    <rdfs:domain rdf:resource="http://example.org/onto/class/azurerm_linux_function_app"/>
    <rdfs:range rdf:resource="http://www.w3.org/2001/XMLSchema#string"/>
  </owl:DatatypeProperty>
  <owl:DatatypeProperty rdf:about="http://example.org/onto/prop/azurerm_linux_function_app_type">
    <rdfs:label>type</rdfs:label>
    <rdfs:comment>Type of database. Possible values include: `MySQL`, `SQLServer`, `SQLAzure`, `Custom`, `NotificationHub`, `ServiceBus`, `EventHub`, `APIHub`, `DocDb`, `RedisCache`, and `PostgreSQL`.</rdfs:comment>
    <rdfs:domain rdf:resource="http://example.org/onto/class/azurerm_linux_function_app"/>
    <rdfs:range rdf:resource="http://www.w3.org/2001/XMLSchema#string"/>
  </owl:DatatypeProperty>
  <owl:DatatypeProperty rdf:about="http://example.org/onto/prop/azurerm_linux_function_app_value">
    <rdfs:label>value</rdfs:label>
    <rdfs:comment>The connection string value.</rdfs:comment>
    <rdfs:domain rdf:resource="http://example.org/onto/class/azurerm_linux_function_app"/>
    <rdfs:range rdf:resource="http://www.w3.org/2001/XMLSchema#string"/>
  </owl:DatatypeProperty>
  <owl:DatatypeProperty rdf:about="http://example.org/onto/prop/azurerm_linux_function_app_identity_ids">
    <rdfs:label>identity_ids</rdfs:label>
    <rdfs:domain rdf:resource="http://example.org/onto/class/azurerm_linux_function_app"/>
    <rdfs:range rdf:resource="http://www.w3.org/2001/XMLSchema#string"/>
  </owl:DatatypeProperty>
  <owl:DatatypeProperty rdf:about="http://example.org/onto/prop/azurerm_linux_function_app_principal_id">
    <rdfs:label>principal_id</rdfs:label>
    <rdfs:domain rdf:resource="http://example.org/onto/class/azurerm_linux_function_app"/>
    <rdfs:range rdf:resource="http://www.w3.org/2001/XMLSchema#string"/>
  </owl:DatatypeProperty>
  <owl:DatatypeProperty rdf:about="http://example.org/onto/prop/azurerm_linux_function_app_tenant_id">
    <rdfs:label>tenant_id</rdfs:label>
    <rdfs:domain rdf:resource="http://example.org/onto/class/azurerm_linux_function_app"/>
    <rdfs:range rdf:resource="http://www.w3.org/2001/XMLSchema#string"/>
  </owl:DatatypeProperty>
  <owl:DatatypeProperty rdf:about="http://example.org/onto/prop/azurerm_linux_function_app_type">
    <rdfs:label>type</rdfs:label>
    <rdfs:domain rdf:resource="http://example.org/onto/class/azurerm_linux_function_app"/>
    <rdfs:range rdf:resource="http://www.w3.org/2001/XMLSchema#string"/>
  </owl:DatatypeProperty>
  <owl:DatatypeProperty rdf:about="http://example.org/onto/prop/azurerm_linux_function_app_always_on">
    <rdfs:label>always_on</rdfs:label>
    <rdfs:comment>If this Linux Web App is Always On enabled. Defaults to `false`.</rdfs:comment>
    <rdfs:domain rdf:resource="http://example.org/onto/class/azurerm_linux_function_app"/>
    <rdfs:range rdf:resource="http://www.w3.org/2001/XMLSchema#string"/>
  </owl:DatatypeProperty>
  <owl:DatatypeProperty rdf:about="http://example.org/onto/prop/azurerm_linux_function_app_api_definition_url">
    <rdfs:label>api_definition_url</rdfs:label>
    <rdfs:comment>The URL of the API definition that describes this Linux Function App.</rdfs:comment>
    <rdfs:domain rdf:resource="http://example.org/onto/class/azurerm_linux_function_app"/>
    <rdfs:range rdf:resource="http://www.w3.org/2001/XMLSchema#string"/>
  </owl:DatatypeProperty>
  <owl:DatatypeProperty rdf:about="http://example.org/onto/prop/azurerm_linux_function_app_api_management_api_id">
    <rdfs:label>api_management_api_id</rdfs:label>
    <rdfs:comment>The ID of the API Management API for this Linux Function App.</rdfs:comment>
    <rdfs:domain rdf:resource="http://example.org/onto/class/azurerm_linux_function_app"/>
    <rdfs:range rdf:resource="http://www.w3.org/2001/XMLSchema#string"/>
  </owl:DatatypeProperty>
  <owl:DatatypeProperty rdf:about="http://example.org/onto/prop/azurerm_linux_function_app_app_command_line">
    <rdfs:label>app_command_line</rdfs:label>
    <rdfs:comment>The program and any arguments used to launch this app via the command line. (Example `node myapp.js`).</rdfs:comment>
    <rdfs:domain rdf:resource="http://example.org/onto/class/azurerm_linux_function_app"/>
    <rdfs:range rdf:resource="http://www.w3.org/2001/XMLSchema#string"/>
  </owl:DatatypeProperty>
  <owl:DatatypeProperty rdf:about="http://example.org/onto/prop/azurerm_linux_function_app_app_scale_limit">
    <rdfs:label>app_scale_limit</rdfs:label>
    <rdfs:comment>The number of workers this function app can scale out to. Only applicable to apps on the Consumption and Premium plan.</rdfs:comment>
    <rdfs:domain rdf:resource="http://example.org/onto/class/azurerm_linux_function_app"/>
    <rdfs:range rdf:resource="http://www.w3.org/2001/XMLSchema#string"/>
  </owl:DatatypeProperty>
  <owl:DatatypeProperty rdf:about="http://example.org/onto/prop/azurerm_linux_function_app_application_insights_connection_string">
    <rdfs:label>application_insights_connection_string</rdfs:label>
    <rdfs:comment>The Connection String for linking the Linux Function App to Application Insights.</rdfs:comment>
    <rdfs:domain rdf:resource="http://example.org/onto/class/azurerm_linux_function_app"/>
    <rdfs:range rdf:resource="http://www.w3.org/2001/XMLSchema#string"/>
  </owl:DatatypeProperty>
  <owl:DatatypeProperty rdf:about="http://example.org/onto/prop/azurerm_linux_function_app_application_insights_key">
    <rdfs:label>application_insights_key</rdfs:label>
    <rdfs:comment>The Instrumentation Key for connecting the Linux Function App to Application Insights.</rdfs:comment>
    <rdfs:domain rdf:resource="http://example.org/onto/class/azurerm_linux_function_app"/>
    <rdfs:range rdf:resource="http://www.w3.org/2001/XMLSchema#string"/>
  </owl:DatatypeProperty>
  <owl:DatatypeProperty rdf:about="http://example.org/onto/prop/azurerm_linux_function_app_container_registry_managed_identity_client_id">
    <rdfs:label>container_registry_managed_identity_client_id</rdfs:label>
    <rdfs:comment>The Client ID of the Managed Service Identity to use for connections to the Azure Container Registry.</rdfs:comment>
    <rdfs:domain rdf:resource="http://example.org/onto/class/azurerm_linux_function_app"/>
    <rdfs:range rdf:resource="http://www.w3.org/2001/XMLSchema#string"/>
  </owl:DatatypeProperty>
  <owl:DatatypeProperty rdf:about="http://example.org/onto/prop/azurerm_linux_function_app_container_registry_use_managed_identity">
    <rdfs:label>container_registry_use_managed_identity</rdfs:label>
    <rdfs:comment>Should connections for Azure Container Registry use Managed Identity.</rdfs:comment>
    <rdfs:domain rdf:resource="http://example.org/onto/class/azurerm_linux_function_app"/>
    <rdfs:range rdf:resource="http://www.w3.org/2001/XMLSchema#string"/>
  </owl:DatatypeProperty>
  <owl:DatatypeProperty rdf:about="http://example.org/onto/prop/azurerm_linux_function_app_default_documents">
    <rdfs:label>default_documents</rdfs:label>
    <rdfs:comment>Specifies a list of Default Documents for the Linux Web App.</rdfs:comment>
    <rdfs:domain rdf:resource="http://example.org/onto/class/azurerm_linux_function_app"/>
    <rdfs:range rdf:resource="http://www.w3.org/2001/XMLSchema#string"/>
  </owl:DatatypeProperty>
  <owl:DatatypeProperty rdf:about="http://example.org/onto/prop/azurerm_linux_function_app_detailed_error_logging_enabled">
    <rdfs:label>detailed_error_logging_enabled</rdfs:label>
    <rdfs:comment>Is detailed error logging enabled</rdfs:comment>
    <rdfs:domain rdf:resource="http://example.org/onto/class/azurerm_linux_function_app"/>
    <rdfs:range rdf:resource="http://www.w3.org/2001/XMLSchema#string"/>
  </owl:DatatypeProperty>
  <owl:DatatypeProperty rdf:about="http://example.org/onto/prop/azurerm_linux_function_app_elastic_instance_minimum">
    <rdfs:label>elastic_instance_minimum</rdfs:label>
    <rdfs:comment>The number of minimum instances for this Linux Function App. Only affects apps on Elastic Premium plans.</rdfs:comment>
    <rdfs:domain rdf:resource="http://example.org/onto/class/azurerm_linux_function_app"/>
    <rdfs:range rdf:resource="http://www.w3.org/2001/XMLSchema#string"/>
  </owl:DatatypeProperty>
  <owl:DatatypeProperty rdf:about="http://example.org/onto/prop/azurerm_linux_function_app_ftps_state">
    <rdfs:label>ftps_state</rdfs:label>
    <rdfs:comment>State of FTP / FTPS service for this function app. Possible values include: `AllAllowed`, `FtpsOnly` and `Disabled`. Defaults to `Disabled`.</rdfs:comment>
    <rdfs:domain rdf:resource="http://example.org/onto/class/azurerm_linux_function_app"/>
    <rdfs:range rdf:resource="http://www.w3.org/2001/XMLSchema#string"/>
  </owl:DatatypeProperty>
  <owl:DatatypeProperty rdf:about="http://example.org/onto/prop/azurerm_linux_function_app_health_check_eviction_time_in_min">
    <rdfs:label>health_check_eviction_time_in_min</rdfs:label>
    <rdfs:comment>The amount of time in minutes that a node is unhealthy before being removed from the load balancer. Possible values are between `2` and `10`. Only valid in conjunction with `health_check_path`</rdfs:comment>
    <rdfs:domain rdf:resource="http://example.org/onto/class/azurerm_linux_function_app"/>
    <rdfs:range rdf:resource="http://www.w3.org/2001/XMLSchema#string"/>
  </owl:DatatypeProperty>
  <owl:DatatypeProperty rdf:about="http://example.org/onto/prop/azurerm_linux_function_app_health_check_path">
    <rdfs:label>health_check_path</rdfs:label>
    <rdfs:comment>The path to be checked for this function app health.</rdfs:comment>
    <rdfs:domain rdf:resource="http://example.org/onto/class/azurerm_linux_function_app"/>
    <rdfs:range rdf:resource="http://www.w3.org/2001/XMLSchema#string"/>
  </owl:DatatypeProperty>
  <owl:DatatypeProperty rdf:about="http://example.org/onto/prop/azurerm_linux_function_app_http2_enabled">
    <rdfs:label>http2_enabled</rdfs:label>
    <rdfs:comment>Specifies if the http2 protocol should be enabled. Defaults to `false`.</rdfs:comment>
    <rdfs:domain rdf:resource="http://example.org/onto/class/azurerm_linux_function_app"/>
    <rdfs:range rdf:resource="http://www.w3.org/2001/XMLSchema#string"/>
  </owl:DatatypeProperty>
  <owl:DatatypeProperty rdf:about="http://example.org/onto/prop/azurerm_linux_function_app_ip_restriction_default_action">
    <rdfs:label>ip_restriction_default_action</rdfs:label>
    <rdfs:domain rdf:resource="http://example.org/onto/class/azurerm_linux_function_app"/>
    <rdfs:range rdf:resource="http://www.w3.org/2001/XMLSchema#string"/>
  </owl:DatatypeProperty>
  <owl:DatatypeProperty rdf:about="http://example.org/onto/prop/azurerm_linux_function_app_linux_fx_version">
    <rdfs:label>linux_fx_version</rdfs:label>
    <rdfs:comment>The Linux FX Version</rdfs:comment>
    <rdfs:domain rdf:resource="http://example.org/onto/class/azurerm_linux_function_app"/>
    <rdfs:range rdf:resource="http://www.w3.org/2001/XMLSchema#string"/>
  </owl:DatatypeProperty>
  <owl:DatatypeProperty rdf:about="http://example.org/onto/prop/azurerm_linux_function_app_load_balancing_mode">
    <rdfs:label>load_balancing_mode</rdfs:label>
    <rdfs:comment>The Site load balancing mode. Possible values include: `WeightedRoundRobin`, `LeastRequests`, `LeastResponseTime`, `WeightedTotalTraffic`, `RequestHash`, `PerSiteRoundRobin`. Defaults to `LeastRequests` if omitted.</rdfs:comment>
    <rdfs:domain rdf:resource="http://example.org/onto/class/azurerm_linux_function_app"/>
    <rdfs:range rdf:resource="http://www.w3.org/2001/XMLSchema#string"/>
  </owl:DatatypeProperty>
  <owl:DatatypeProperty rdf:about="http://example.org/onto/prop/azurerm_linux_function_app_managed_pipeline_mode">
    <rdfs:label>managed_pipeline_mode</rdfs:label>
    <rdfs:comment>The Managed Pipeline mode. Possible values include: `Integrated`, `Classic`. Defaults to `Integrated`.</rdfs:comment>
    <rdfs:domain rdf:resource="http://example.org/onto/class/azurerm_linux_function_app"/>
    <rdfs:range rdf:resource="http://www.w3.org/2001/XMLSchema#string"/>
  </owl:DatatypeProperty>
  <owl:DatatypeProperty rdf:about="http://example.org/onto/prop/azurerm_linux_function_app_minimum_tls_version">
    <rdfs:label>minimum_tls_version</rdfs:label>
    <rdfs:comment>The configures the minimum version of TLS required for SSL requests. Possible values include: `1.0`, `1.1`, and  `1.2`. Defaults to `1.2`.</rdfs:comment>
    <rdfs:domain rdf:resource="http://example.org/onto/class/azurerm_linux_function_app"/>
    <rdfs:range rdf:resource="http://www.w3.org/2001/XMLSchema#string"/>
  </owl:DatatypeProperty>
  <owl:DatatypeProperty rdf:about="http://example.org/onto/prop/azurerm_linux_function_app_pre_warmed_instance_count">
    <rdfs:label>pre_warmed_instance_count</rdfs:label>
    <rdfs:comment>The number of pre-warmed instances for this function app. Only affects apps on an Elastic Premium plan.</rdfs:comment>
    <rdfs:domain rdf:resource="http://example.org/onto/class/azurerm_linux_function_app"/>
    <rdfs:range rdf:resource="http://www.w3.org/2001/XMLSchema#string"/>
  </owl:DatatypeProperty>
  <owl:DatatypeProperty rdf:about="http://example.org/onto/prop/azurerm_linux_function_app_remote_debugging_enabled">
    <rdfs:label>remote_debugging_enabled</rdfs:label>
    <rdfs:comment>Should Remote Debugging be enabled. Defaults to `false`.</rdfs:comment>
    <rdfs:domain rdf:resource="http://example.org/onto/class/azurerm_linux_function_app"/>
    <rdfs:range rdf:resource="http://www.w3.org/2001/XMLSchema#string"/>
  </owl:DatatypeProperty>
  <owl:DatatypeProperty rdf:about="http://example.org/onto/prop/azurerm_linux_function_app_remote_debugging_version">
    <rdfs:label>remote_debugging_version</rdfs:label>
    <rdfs:comment>The Remote Debugging Version. Currently only `VS2022` is supported.</rdfs:comment>
    <rdfs:domain rdf:resource="http://example.org/onto/class/azurerm_linux_function_app"/>
    <rdfs:range rdf:resource="http://www.w3.org/2001/XMLSchema#string"/>
  </owl:DatatypeProperty>
  <owl:DatatypeProperty rdf:about="http://example.org/onto/prop/azurerm_linux_function_app_runtime_scale_monitoring_enabled">
    <rdfs:label>runtime_scale_monitoring_enabled</rdfs:label>
    <rdfs:comment>Should Functions Runtime Scale Monitoring be enabled.</rdfs:comment>
    <rdfs:domain rdf:resource="http://example.org/onto/class/azurerm_linux_function_app"/>
    <rdfs:range rdf:resource="http://www.w3.org/2001/XMLSchema#string"/>
  </owl:DatatypeProperty>
  <owl:DatatypeProperty rdf:about="http://example.org/onto/prop/azurerm_linux_function_app_scm_ip_restriction_default_action">
    <rdfs:label>scm_ip_restriction_default_action</rdfs:label>
    <rdfs:domain rdf:resource="http://example.org/onto/class/azurerm_linux_function_app"/>
    <rdfs:range rdf:resource="http://www.w3.org/2001/XMLSchema#string"/>
  </owl:DatatypeProperty>
  <owl:DatatypeProperty rdf:about="http://example.org/onto/prop/azurerm_linux_function_app_scm_minimum_tls_version">
    <rdfs:label>scm_minimum_tls_version</rdfs:label>
    <rdfs:comment>Configures the minimum version of TLS required for SSL requests to the SCM site Possible values include: `1.0`, `1.1`, `1.2` and  `1.3`. Defaults to `1.2`.</rdfs:comment>
    <rdfs:domain rdf:resource="http://example.org/onto/class/azurerm_linux_function_app"/>
    <rdfs:range rdf:resource="http://www.w3.org/2001/XMLSchema#string"/>
  </owl:DatatypeProperty>
  <owl:DatatypeProperty rdf:about="http://example.org/onto/prop/azurerm_linux_function_app_scm_type">
    <rdfs:label>scm_type</rdfs:label>
    <rdfs:comment>The SCM Type in use by the Linux Function App.</rdfs:comment>
    <rdfs:domain rdf:resource="http://example.org/onto/class/azurerm_linux_function_app"/>
    <rdfs:range rdf:resource="http://www.w3.org/2001/XMLSchema#string"/>
  </owl:DatatypeProperty>
  <owl:DatatypeProperty rdf:about="http://example.org/onto/prop/azurerm_linux_function_app_scm_use_main_ip_restriction">
    <rdfs:label>scm_use_main_ip_restriction</rdfs:label>
    <rdfs:comment>Should the Linux Function App `ip_restriction` configuration be used for the SCM also.</rdfs:comment>
    <rdfs:domain rdf:resource="http://example.org/onto/class/azurerm_linux_function_app"/>
    <rdfs:range rdf:resource="http://www.w3.org/2001/XMLSchema#string"/>
  </owl:DatatypeProperty>
  <owl:DatatypeProperty rdf:about="http://example.org/onto/prop/azurerm_linux_function_app_use_32_bit_worker">
    <rdfs:label>use_32_bit_worker</rdfs:label>
    <rdfs:comment>Should the Linux Web App use a 32-bit worker.</rdfs:comment>
    <rdfs:domain rdf:resource="http://example.org/onto/class/azurerm_linux_function_app"/>
    <rdfs:range rdf:resource="http://www.w3.org/2001/XMLSchema#string"/>
  </owl:DatatypeProperty>
  <owl:DatatypeProperty rdf:about="http://example.org/onto/prop/azurerm_linux_function_app_vnet_route_all_enabled">
    <rdfs:label>vnet_route_all_enabled</rdfs:label>
    <rdfs:comment>Should all outbound traffic to have Virtual Network Security Groups and User Defined Routes applied? Defaults to `false`.</rdfs:comment>
    <rdfs:domain rdf:resource="http://example.org/onto/class/azurerm_linux_function_app"/>
    <rdfs:range rdf:resource="http://www.w3.org/2001/XMLSchema#string"/>
  </owl:DatatypeProperty>
  <owl:DatatypeProperty rdf:about="http://example.org/onto/prop/azurerm_linux_function_app_websockets_enabled">
    <rdfs:label>websockets_enabled</rdfs:label>
    <rdfs:comment>Should Web Sockets be enabled. Defaults to `false`.</rdfs:comment>
    <rdfs:domain rdf:resource="http://example.org/onto/class/azurerm_linux_function_app"/>
    <rdfs:range rdf:resource="http://www.w3.org/2001/XMLSchema#string"/>
  </owl:DatatypeProperty>
  <owl:DatatypeProperty rdf:about="http://example.org/onto/prop/azurerm_linux_function_app_worker_count">
    <rdfs:label>worker_count</rdfs:label>
    <rdfs:comment>The number of Workers for this Linux Function App.</rdfs:comment>
    <rdfs:domain rdf:resource="http://example.org/onto/class/azurerm_linux_function_app"/>
    <rdfs:range rdf:resource="http://www.w3.org/2001/XMLSchema#string"/>
  </owl:DatatypeProperty>
  <owl:DatatypeProperty rdf:about="http://example.org/onto/prop/azurerm_linux_function_app_disk_quota_mb">
    <rdfs:label>disk_quota_mb</rdfs:label>
    <rdfs:comment>The amount of disk space to use for logs. Valid values are between `25` and `100`.</rdfs:comment>
    <rdfs:domain rdf:resource="http://example.org/onto/class/azurerm_linux_function_app"/>
    <rdfs:range rdf:resource="http://www.w3.org/2001/XMLSchema#string"/>
  </owl:DatatypeProperty>
  <owl:DatatypeProperty rdf:about="http://example.org/onto/prop/azurerm_linux_function_app_retention_period_days">
    <rdfs:label>retention_period_days</rdfs:label>
    <rdfs:comment>The retention period for logs in days. Valid values are between `0` and `99999`. Defaults to `0` (never delete).</rdfs:comment>
    <rdfs:domain rdf:resource="http://example.org/onto/class/azurerm_linux_function_app"/>
    <rdfs:range rdf:resource="http://www.w3.org/2001/XMLSchema#string"/>
  </owl:DatatypeProperty>
  <owl:DatatypeProperty rdf:about="http://example.org/onto/prop/azurerm_linux_function_app_dotnet_version">
    <rdfs:label>dotnet_version</rdfs:label>
    <rdfs:comment>The version of .Net. Possible values are `3.1`, `6.0`, `7.0`, `8.0` and `9.0`</rdfs:comment>
    <rdfs:domain rdf:resource="http://example.org/onto/class/azurerm_linux_function_app"/>
    <rdfs:range rdf:resource="http://www.w3.org/2001/XMLSchema#string"/>
  </owl:DatatypeProperty>
  <owl:DatatypeProperty rdf:about="http://example.org/onto/prop/azurerm_linux_function_app_java_version">
    <rdfs:label>java_version</rdfs:label>
    <rdfs:comment>The version of Java to use. Possible values are `8`, `11`, `17`, and `21`</rdfs:comment>
    <rdfs:domain rdf:resource="http://example.org/onto/class/azurerm_linux_function_app"/>
    <rdfs:range rdf:resource="http://www.w3.org/2001/XMLSchema#string"/>
  </owl:DatatypeProperty>
  <owl:DatatypeProperty rdf:about="http://example.org/onto/prop/azurerm_linux_function_app_node_version">
    <rdfs:label>node_version</rdfs:label>
    <rdfs:comment>The version of Node to use. Possible values include `12`, `14`, `16`, `18`, `20` and `22`</rdfs:comment>
    <rdfs:domain rdf:resource="http://example.org/onto/class/azurerm_linux_function_app"/>
    <rdfs:range rdf:resource="http://www.w3.org/2001/XMLSchema#string"/>
  </owl:DatatypeProperty>
  <owl:DatatypeProperty rdf:about="http://example.org/onto/prop/azurerm_linux_function_app_powershell_core_version">
    <rdfs:label>powershell_core_version</rdfs:label>
    <rdfs:comment>The version of PowerShell Core to use. Possibles values are `7`, `7.2`, and `7.4`</rdfs:comment>
    <rdfs:domain rdf:resource="http://example.org/onto/class/azurerm_linux_function_app"/>
    <rdfs:range rdf:resource="http://www.w3.org/2001/XMLSchema#string"/>
  </owl:DatatypeProperty>
  <owl:DatatypeProperty rdf:about="http://example.org/onto/prop/azurerm_linux_function_app_python_version">
    <rdfs:label>python_version</rdfs:label>
    <rdfs:comment>The version of Python to use. Possible values include `3.13`, `3.12`, `3.11`, `3.10`, `3.9`, `3.8`, and `3.7`.</rdfs:comment>
    <rdfs:domain rdf:resource="http://example.org/onto/class/azurerm_linux_function_app"/>
    <rdfs:range rdf:resource="http://www.w3.org/2001/XMLSchema#string"/>
  </owl:DatatypeProperty>
  <owl:DatatypeProperty rdf:about="http://example.org/onto/prop/azurerm_linux_function_app_use_custom_runtime">
    <rdfs:label>use_custom_runtime</rdfs:label>
    <rdfs:domain rdf:resource="http://example.org/onto/class/azurerm_linux_function_app"/>
    <rdfs:range rdf:resource="http://www.w3.org/2001/XMLSchema#string"/>
  </owl:DatatypeProperty>
  <owl:DatatypeProperty rdf:about="http://example.org/onto/prop/azurerm_linux_function_app_use_dotnet_isolated_runtime">
    <rdfs:label>use_dotnet_isolated_runtime</rdfs:label>
    <rdfs:comment>Should the DotNet process use an isolated runtime. Defaults to `false`.</rdfs:comment>
    <rdfs:domain rdf:resource="http://example.org/onto/class/azurerm_linux_function_app"/>
    <rdfs:range rdf:resource="http://www.w3.org/2001/XMLSchema#string"/>
  </owl:DatatypeProperty>
  <owl:DatatypeProperty rdf:about="http://example.org/onto/prop/azurerm_linux_function_app_image_name">
    <rdfs:label>image_name</rdfs:label>
    <rdfs:comment>The name of the Docker image to use.</rdfs:comment>
    <rdfs:domain rdf:resource="http://example.org/onto/class/azurerm_linux_function_app"/>
    <rdfs:range rdf:resource="http://www.w3.org/2001/XMLSchema#string"/>
  </owl:DatatypeProperty>
  <owl:DatatypeProperty rdf:about="http://example.org/onto/prop/azurerm_linux_function_app_image_tag">
    <rdfs:label>image_tag</rdfs:label>
    <rdfs:comment>The image tag of the image to use.</rdfs:comment>
    <rdfs:domain rdf:resource="http://example.org/onto/class/azurerm_linux_function_app"/>
    <rdfs:range rdf:resource="http://www.w3.org/2001/XMLSchema#string"/>
  </owl:DatatypeProperty>
  <owl:DatatypeProperty rdf:about="http://example.org/onto/prop/azurerm_linux_function_app_registry_password">
    <rdfs:label>registry_password</rdfs:label>
    <rdfs:comment>The password for the account to use to connect to the registry.</rdfs:comment>
    <rdfs:domain rdf:resource="http://example.org/onto/class/azurerm_linux_function_app"/>
    <rdfs:range rdf:resource="http://www.w3.org/2001/XMLSchema#string"/>
  </owl:DatatypeProperty>
  <owl:DatatypeProperty rdf:about="http://example.org/onto/prop/azurerm_linux_function_app_registry_url">
    <rdfs:label>registry_url</rdfs:label>
    <rdfs:comment>The URL of the docker registry.</rdfs:comment>
    <rdfs:domain rdf:resource="http://example.org/onto/class/azurerm_linux_function_app"/>
    <rdfs:range rdf:resource="http://www.w3.org/2001/XMLSchema#string"/>
  </owl:DatatypeProperty>
  <owl:DatatypeProperty rdf:about="http://example.org/onto/prop/azurerm_linux_function_app_registry_username">
    <rdfs:label>registry_username</rdfs:label>
    <rdfs:comment>The username to use for connections to the registry.</rdfs:comment>
    <rdfs:domain rdf:resource="http://example.org/onto/class/azurerm_linux_function_app"/>
    <rdfs:range rdf:resource="http://www.w3.org/2001/XMLSchema#string"/>
  </owl:DatatypeProperty>
  <owl:DatatypeProperty rdf:about="http://example.org/onto/prop/azurerm_linux_function_app_allowed_origins">
    <rdfs:label>allowed_origins</rdfs:label>
    <rdfs:comment>Specifies a list of origins that should be allowed to make cross-origin calls.</rdfs:comment>
    <rdfs:domain rdf:resource="http://example.org/onto/class/azurerm_linux_function_app"/>
    <rdfs:range rdf:resource="http://www.w3.org/2001/XMLSchema#string"/>
  </owl:DatatypeProperty>
  <owl:DatatypeProperty rdf:about="http://example.org/onto/prop/azurerm_linux_function_app_support_credentials">
    <rdfs:label>support_credentials</rdfs:label>
    <rdfs:comment>Are credentials allowed in CORS requests? Defaults to `false`.</rdfs:comment>
    <rdfs:domain rdf:resource="http://example.org/onto/class/azurerm_linux_function_app"/>
    <rdfs:range rdf:resource="http://www.w3.org/2001/XMLSchema#string"/>
  </owl:DatatypeProperty>
  <owl:DatatypeProperty rdf:about="http://example.org/onto/prop/azurerm_linux_function_app_action">
    <rdfs:label>action</rdfs:label>
    <rdfs:comment>The action to take. Possible values are `Allow` or `Deny`.</rdfs:comment>
    <rdfs:domain rdf:resource="http://example.org/onto/class/azurerm_linux_function_app"/>
    <rdfs:range rdf:resource="http://www.w3.org/2001/XMLSchema#string"/>
  </owl:DatatypeProperty>
  <owl:DatatypeProperty rdf:about="http://example.org/onto/prop/azurerm_linux_function_app_description">
    <rdfs:label>description</rdfs:label>
    <rdfs:comment>The description of the IP restriction rule.</rdfs:comment>
    <rdfs:domain rdf:resource="http://example.org/onto/class/azurerm_linux_function_app"/>
    <rdfs:range rdf:resource="http://www.w3.org/2001/XMLSchema#string"/>
  </owl:DatatypeProperty>
  <owl:DatatypeProperty rdf:about="http://example.org/onto/prop/azurerm_linux_function_app_headers">
    <rdfs:label>headers</rdfs:label>
    <rdfs:domain rdf:resource="http://example.org/onto/class/azurerm_linux_function_app"/>
    <rdfs:range rdf:resource="http://www.w3.org/2001/XMLSchema#string"/>
  </owl:DatatypeProperty>
  <owl:DatatypeProperty rdf:about="http://example.org/onto/prop/azurerm_linux_function_app_ip_address">
    <rdfs:label>ip_address</rdfs:label>
    <rdfs:comment>The CIDR notation of the IP or IP Range to match. For example: `10.0.0.0/24` or `192.168.10.1/32` or `fe80::/64` or `13.107.6.152/31,13.107.128.0/22`</rdfs:comment>
    <rdfs:domain rdf:resource="http://example.org/onto/class/azurerm_linux_function_app"/>
    <rdfs:range rdf:resource="http://www.w3.org/2001/XMLSchema#string"/>
  </owl:DatatypeProperty>
  <owl:DatatypeProperty rdf:about="http://example.org/onto/prop/azurerm_linux_function_app_name">
    <rdfs:label>name</rdfs:label>
    <rdfs:comment>The name which should be used for this `ip_restriction`.</rdfs:comment>
    <rdfs:domain rdf:resource="http://example.org/onto/class/azurerm_linux_function_app"/>
    <rdfs:range rdf:resource="http://www.w3.org/2001/XMLSchema#string"/>
  </owl:DatatypeProperty>
  <owl:DatatypeProperty rdf:about="http://example.org/onto/prop/azurerm_linux_function_app_priority">
    <rdfs:label>priority</rdfs:label>
    <rdfs:comment>The priority value of this `ip_restriction`.</rdfs:comment>
    <rdfs:domain rdf:resource="http://example.org/onto/class/azurerm_linux_function_app"/>
    <rdfs:range rdf:resource="http://www.w3.org/2001/XMLSchema#string"/>
  </owl:DatatypeProperty>
  <owl:DatatypeProperty rdf:about="http://example.org/onto/prop/azurerm_linux_function_app_service_tag">
    <rdfs:label>service_tag</rdfs:label>
    <rdfs:comment>The Service Tag used for this IP Restriction.</rdfs:comment>
    <rdfs:domain rdf:resource="http://example.org/onto/class/azurerm_linux_function_app"/>
    <rdfs:range rdf:resource="http://www.w3.org/2001/XMLSchema#string"/>
  </owl:DatatypeProperty>
  <owl:DatatypeProperty rdf:about="http://example.org/onto/prop/azurerm_linux_function_app_virtual_network_subnet_id">
    <rdfs:label>virtual_network_subnet_id</rdfs:label>
    <rdfs:comment>The Virtual Network Subnet ID used for this IP Restriction.</rdfs:comment>
    <rdfs:domain rdf:resource="http://example.org/onto/class/azurerm_linux_function_app"/>
    <rdfs:range rdf:resource="http://www.w3.org/2001/XMLSchema#string"/>
  </owl:DatatypeProperty>
  <owl:DatatypeProperty rdf:about="http://example.org/onto/prop/azurerm_linux_function_app_action">
    <rdfs:label>action</rdfs:label>
    <rdfs:comment>The action to take. Possible values are `Allow` or `Deny`.</rdfs:comment>
    <rdfs:domain rdf:resource="http://example.org/onto/class/azurerm_linux_function_app"/>
    <rdfs:range rdf:resource="http://www.w3.org/2001/XMLSchema#string"/>
  </owl:DatatypeProperty>
  <owl:DatatypeProperty rdf:about="http://example.org/onto/prop/azurerm_linux_function_app_description">
    <rdfs:label>description</rdfs:label>
    <rdfs:comment>The description of the IP restriction rule.</rdfs:comment>
    <rdfs:domain rdf:resource="http://example.org/onto/class/azurerm_linux_function_app"/>
    <rdfs:range rdf:resource="http://www.w3.org/2001/XMLSchema#string"/>
  </owl:DatatypeProperty>
  <owl:DatatypeProperty rdf:about="http://example.org/onto/prop/azurerm_linux_function_app_headers">
    <rdfs:label>headers</rdfs:label>
    <rdfs:domain rdf:resource="http://example.org/onto/class/azurerm_linux_function_app"/>
    <rdfs:range rdf:resource="http://www.w3.org/2001/XMLSchema#string"/>
  </owl:DatatypeProperty>
  <owl:DatatypeProperty rdf:about="http://example.org/onto/prop/azurerm_linux_function_app_ip_address">
    <rdfs:label>ip_address</rdfs:label>
    <rdfs:comment>The CIDR notation of the IP or IP Range to match. For example: `10.0.0.0/24` or `192.168.10.1/32` or `fe80::/64` or `13.107.6.152/31,13.107.128.0/22`</rdfs:comment>
    <rdfs:domain rdf:resource="http://example.org/onto/class/azurerm_linux_function_app"/>
    <rdfs:range rdf:resource="http://www.w3.org/2001/XMLSchema#string"/>
  </owl:DatatypeProperty>
  <owl:DatatypeProperty rdf:about="http://example.org/onto/prop/azurerm_linux_function_app_name">
    <rdfs:label>name</rdfs:label>
    <rdfs:comment>The name which should be used for this `ip_restriction`.</rdfs:comment>
    <rdfs:domain rdf:resource="http://example.org/onto/class/azurerm_linux_function_app"/>
    <rdfs:range rdf:resource="http://www.w3.org/2001/XMLSchema#string"/>
  </owl:DatatypeProperty>
  <owl:DatatypeProperty rdf:about="http://example.org/onto/prop/azurerm_linux_function_app_priority">
    <rdfs:label>priority</rdfs:label>
    <rdfs:comment>The priority value of this `ip_restriction`.</rdfs:comment>
    <rdfs:domain rdf:resource="http://example.org/onto/class/azurerm_linux_function_app"/>
    <rdfs:range rdf:resource="http://www.w3.org/2001/XMLSchema#string"/>
  </owl:DatatypeProperty>
  <owl:DatatypeProperty rdf:about="http://example.org/onto/prop/azurerm_linux_function_app_service_tag">
    <rdfs:label>service_tag</rdfs:label>
    <rdfs:comment>The Service Tag used for this IP Restriction.</rdfs:comment>
    <rdfs:domain rdf:resource="http://example.org/onto/class/azurerm_linux_function_app"/>
    <rdfs:range rdf:resource="http://www.w3.org/2001/XMLSchema#string"/>
  </owl:DatatypeProperty>
  <owl:DatatypeProperty rdf:about="http://example.org/onto/prop/azurerm_linux_function_app_virtual_network_subnet_id">
    <rdfs:label>virtual_network_subnet_id</rdfs:label>
    <rdfs:comment>The Virtual Network Subnet ID used for this IP Restriction.</rdfs:comment>
    <rdfs:domain rdf:resource="http://example.org/onto/class/azurerm_linux_function_app"/>
    <rdfs:range rdf:resource="http://www.w3.org/2001/XMLSchema#string"/>
  </owl:DatatypeProperty>
  <owl:DatatypeProperty rdf:about="http://example.org/onto/prop/azurerm_linux_function_app_app_setting_names">
    <rdfs:label>app_setting_names</rdfs:label>
    <rdfs:domain rdf:resource="http://example.org/onto/class/azurerm_linux_function_app"/>
    <rdfs:range rdf:resource="http://www.w3.org/2001/XMLSchema#string"/>
  </owl:DatatypeProperty>
  <owl:DatatypeProperty rdf:about="http://example.org/onto/prop/azurerm_linux_function_app_connection_string_names">
    <rdfs:label>connection_string_names</rdfs:label>
    <rdfs:domain rdf:resource="http://example.org/onto/class/azurerm_linux_function_app"/>
    <rdfs:range rdf:resource="http://www.w3.org/2001/XMLSchema#string"/>
  </owl:DatatypeProperty>
  <owl:DatatypeProperty rdf:about="http://example.org/onto/prop/azurerm_linux_function_app_access_key">
    <rdfs:label>access_key</rdfs:label>
    <rdfs:domain rdf:resource="http://example.org/onto/class/azurerm_linux_function_app"/>
    <rdfs:range rdf:resource="http://www.w3.org/2001/XMLSchema#string"/>
  </owl:DatatypeProperty>
  <owl:DatatypeProperty rdf:about="http://example.org/onto/prop/azurerm_linux_function_app_account_name">
    <rdfs:label>account_name</rdfs:label>
    <rdfs:domain rdf:resource="http://example.org/onto/class/azurerm_linux_function_app"/>
    <rdfs:range rdf:resource="http://www.w3.org/2001/XMLSchema#string"/>
  </owl:DatatypeProperty>
  <owl:DatatypeProperty rdf:about="http://example.org/onto/prop/azurerm_linux_function_app_mount_path">
    <rdfs:label>mount_path</rdfs:label>
    <rdfs:domain rdf:resource="http://example.org/onto/class/azurerm_linux_function_app"/>
    <rdfs:range rdf:resource="http://www.w3.org/2001/XMLSchema#string"/>
  </owl:DatatypeProperty>
  <owl:DatatypeProperty rdf:about="http://example.org/onto/prop/azurerm_linux_function_app_name">
    <rdfs:label>name</rdfs:label>
    <rdfs:domain rdf:resource="http://example.org/onto/class/azurerm_linux_function_app"/>
    <rdfs:range rdf:resource="http://www.w3.org/2001/XMLSchema#string"/>
  </owl:DatatypeProperty>
  <owl:DatatypeProperty rdf:about="http://example.org/onto/prop/azurerm_linux_function_app_share_name">
    <rdfs:label>share_name</rdfs:label>
    <rdfs:domain rdf:resource="http://example.org/onto/class/azurerm_linux_function_app"/>
    <rdfs:range rdf:resource="http://www.w3.org/2001/XMLSchema#string"/>
  </owl:DatatypeProperty>
  <owl:DatatypeProperty rdf:about="http://example.org/onto/prop/azurerm_linux_function_app_type">
    <rdfs:label>type</rdfs:label>
    <rdfs:domain rdf:resource="http://example.org/onto/class/azurerm_linux_function_app"/>
    <rdfs:range rdf:resource="http://www.w3.org/2001/XMLSchema#string"/>
  </owl:DatatypeProperty>
  <owl:DatatypeProperty rdf:about="http://example.org/onto/prop/azurerm_linux_function_app_create">
    <rdfs:label>create</rdfs:label>
    <rdfs:domain rdf:resource="http://example.org/onto/class/azurerm_linux_function_app"/>
    <rdfs:range rdf:resource="http://www.w3.org/2001/XMLSchema#string"/>
  </owl:DatatypeProperty>
  <owl:DatatypeProperty rdf:about="http://example.org/onto/prop/azurerm_linux_function_app_delete">
    <rdfs:label>delete</rdfs:label>
    <rdfs:domain rdf:resource="http://example.org/onto/class/azurerm_linux_function_app"/>
    <rdfs:range rdf:resource="http://www.w3.org/2001/XMLSchema#string"/>
  </owl:DatatypeProperty>
  <owl:DatatypeProperty rdf:about="http://example.org/onto/prop/azurerm_linux_function_app_read">
    <rdfs:label>read</rdfs:label>
    <rdfs:domain rdf:resource="http://example.org/onto/class/azurerm_linux_function_app"/>
    <rdfs:range rdf:resource="http://www.w3.org/2001/XMLSchema#string"/>
  </owl:DatatypeProperty>
  <owl:DatatypeProperty rdf:about="http://example.org/onto/prop/azurerm_linux_function_app_update">
    <rdfs:label>update</rdfs:label>
    <rdfs:domain rdf:resource="http://example.org/onto/class/azurerm_linux_function_app"/>
    <rdfs:range rdf:resource="http://www.w3.org/2001/XMLSchema#string"/>
  </owl:DatatypeProperty>
</rdf:RDF>
