<?xml version="1.0" encoding="UTF-8"?>
<rdf:RDF
  xmlns:rdf="http://www.w3.org/1999/02/22-rdf-syntax-ns#"
  xmlns:rdfs="http://www.w3.org/2000/01/rdf-schema#"
  xmlns:owl="http://www.w3.org/2002/07/owl#"
  xmlns:xsd="http://www.w3.org/2001/XMLSchema#"
  xml:base="http://example.org/onto/">
  <owl:Class rdf:about="http://example.org/onto/class/google_kms_crypto_key">
    <rdfs:label>google_kms_crypto_key</rdfs:label>
    <rdfs:comment>#
#     ***     AUTO GENERATED CODE    ***    Type: MMv1     ***
#
# ----------------------------------------------------------------------------
#
#     This code is generated by Magic Modules using the following:
#
#     Configuration: https:#github.com/GoogleCloudPlatform/magic-modules/tree/main/mmv1/products/kms/CryptoKey.yaml
#     Template:      https:#github.com/GoogleCloudPlatform/magic-modules/tree/main/mmv1/templates/terraform/resource.html.markdown.tmpl
#
#     DO NOT EDIT this file directly. Any changes made to this file will be
#     overwritten during the next generation cycle.
#
# ----------------------------------------------------------------------------
subcategory: "Cloud Key Management Service"
description: |-
  A `CryptoKey` represents a logical key that can be used for cryptographic operations.
---</rdfs:comment>
  </owl:Class>
  <owl:DatatypeProperty rdf:about="http://example.org/onto/prop/google_kms_crypto_key_crypto_key_backend">
    <rdfs:label>crypto_key_backend</rdfs:label>
    <rdfs:comment>The resource name of the backend environment associated with all CryptoKeyVersions within this CryptoKey.
The resource name is in the format "projects/*/locations/*/ekmConnections/*" and only applies to "EXTERNAL_VPC" keys.</rdfs:comment>
    <rdfs:domain rdf:resource="http://example.org/onto/class/google_kms_crypto_key"/>
    <rdfs:range rdf:resource="http://www.w3.org/2001/XMLSchema#string"/>
  </owl:DatatypeProperty>
  <owl:DatatypeProperty rdf:about="http://example.org/onto/prop/google_kms_crypto_key_destroy_scheduled_duration">
    <rdfs:label>destroy_scheduled_duration</rdfs:label>
    <rdfs:comment>The period of time that versions of this key spend in the DESTROY_SCHEDULED state before transitioning to DESTROYED.
If not specified at creation time, the default duration is 30 days.</rdfs:comment>
    <rdfs:domain rdf:resource="http://example.org/onto/class/google_kms_crypto_key"/>
    <rdfs:range rdf:resource="http://www.w3.org/2001/XMLSchema#string"/>
  </owl:DatatypeProperty>
  <owl:DatatypeProperty rdf:about="http://example.org/onto/prop/google_kms_crypto_key_effective_labels">
    <rdfs:label>effective_labels</rdfs:label>
    <rdfs:comment>All of labels (key/value pairs) present on the resource in GCP, including the labels configured through Terraform, other clients and services.</rdfs:comment>
    <rdfs:domain rdf:resource="http://example.org/onto/class/google_kms_crypto_key"/>
    <rdfs:range rdf:resource="http://www.w3.org/2001/XMLSchema#string"/>
  </owl:DatatypeProperty>
  <owl:DatatypeProperty rdf:about="http://example.org/onto/prop/google_kms_crypto_key_id">
    <rdfs:label>id</rdfs:label>
    <rdfs:domain rdf:resource="http://example.org/onto/class/google_kms_crypto_key"/>
    <rdfs:range rdf:resource="http://www.w3.org/2001/XMLSchema#string"/>
  </owl:DatatypeProperty>
  <owl:DatatypeProperty rdf:about="http://example.org/onto/prop/google_kms_crypto_key_import_only">
    <rdfs:label>import_only</rdfs:label>
    <rdfs:comment>Whether this key may contain imported versions only.</rdfs:comment>
    <rdfs:domain rdf:resource="http://example.org/onto/class/google_kms_crypto_key"/>
    <rdfs:range rdf:resource="http://www.w3.org/2001/XMLSchema#string"/>
  </owl:DatatypeProperty>
  <owl:DatatypeProperty rdf:about="http://example.org/onto/prop/google_kms_crypto_key_key_ring">
    <rdfs:label>key_ring</rdfs:label>
    <rdfs:comment>The KeyRing that this key belongs to.
Format: ''projects/{{project}}/locations/{{location}}/keyRings/{{keyRing}}''.</rdfs:comment>
    <rdfs:domain rdf:resource="http://example.org/onto/class/google_kms_crypto_key"/>
    <rdfs:range rdf:resource="http://www.w3.org/2001/XMLSchema#string"/>
  </owl:DatatypeProperty>
  <owl:DatatypeProperty rdf:about="http://example.org/onto/prop/google_kms_crypto_key_labels">
    <rdfs:label>labels</rdfs:label>
    <rdfs:comment>Labels with user-defined metadata to apply to this resource.


**Note**: This field is non-authoritative, and will only manage the labels present in your configuration.
Please refer to the field 'effective_labels' for all of the labels present on the resource.</rdfs:comment>
    <rdfs:domain rdf:resource="http://example.org/onto/class/google_kms_crypto_key"/>
    <rdfs:range rdf:resource="http://www.w3.org/2001/XMLSchema#string"/>
  </owl:DatatypeProperty>
  <owl:DatatypeProperty rdf:about="http://example.org/onto/prop/google_kms_crypto_key_name">
    <rdfs:label>name</rdfs:label>
    <rdfs:comment>The resource name for the CryptoKey.</rdfs:comment>
    <rdfs:domain rdf:resource="http://example.org/onto/class/google_kms_crypto_key"/>
    <rdfs:range rdf:resource="http://www.w3.org/2001/XMLSchema#string"/>
  </owl:DatatypeProperty>
  <owl:DatatypeProperty rdf:about="http://example.org/onto/prop/google_kms_crypto_key_primary">
    <rdfs:label>primary</rdfs:label>
    <rdfs:comment>A copy of the primary CryptoKeyVersion that will be used by cryptoKeys.encrypt when this CryptoKey is given in EncryptRequest.name.
Keys with purpose ENCRYPT_DECRYPT may have a primary. For other keys, this field will be unset.</rdfs:comment>
    <rdfs:domain rdf:resource="http://example.org/onto/class/google_kms_crypto_key"/>
    <rdfs:range rdf:resource="http://www.w3.org/2001/XMLSchema#string"/>
  </owl:DatatypeProperty>
  <owl:DatatypeProperty rdf:about="http://example.org/onto/prop/google_kms_crypto_key_purpose">
    <rdfs:label>purpose</rdfs:label>
    <rdfs:comment>The immutable purpose of this CryptoKey. See the
[purpose reference](https://cloud.google.com/kms/docs/reference/rest/v1/projects.locations.keyRings.cryptoKeys#CryptoKeyPurpose)
for possible inputs.
Default value is "ENCRYPT_DECRYPT".</rdfs:comment>
    <rdfs:domain rdf:resource="http://example.org/onto/class/google_kms_crypto_key"/>
    <rdfs:range rdf:resource="http://www.w3.org/2001/XMLSchema#string"/>
  </owl:DatatypeProperty>
  <owl:DatatypeProperty rdf:about="http://example.org/onto/prop/google_kms_crypto_key_rotation_period">
    <rdfs:label>rotation_period</rdfs:label>
    <rdfs:comment>Every time this period passes, generate a new CryptoKeyVersion and set it as the primary.
The first rotation will take place after the specified period. The rotation period has
the format of a decimal number with up to 9 fractional digits, followed by the
letter 's' (seconds). It must be greater than a day (ie, 86400).</rdfs:comment>
    <rdfs:domain rdf:resource="http://example.org/onto/class/google_kms_crypto_key"/>
    <rdfs:range rdf:resource="http://www.w3.org/2001/XMLSchema#string"/>
  </owl:DatatypeProperty>
  <owl:DatatypeProperty rdf:about="http://example.org/onto/prop/google_kms_crypto_key_skip_initial_version_creation">
    <rdfs:label>skip_initial_version_creation</rdfs:label>
    <rdfs:comment>If set to true, the request will create a CryptoKey without any CryptoKeyVersions.
You must use the 'google_kms_crypto_key_version' resource to create a new CryptoKeyVersion
or 'google_kms_key_ring_import_job' resource to import the CryptoKeyVersion.
This field is only applicable during initial CryptoKey creation.</rdfs:comment>
    <rdfs:domain rdf:resource="http://example.org/onto/class/google_kms_crypto_key"/>
    <rdfs:range rdf:resource="http://www.w3.org/2001/XMLSchema#string"/>
  </owl:DatatypeProperty>
  <owl:DatatypeProperty rdf:about="http://example.org/onto/prop/google_kms_crypto_key_terraform_labels">
    <rdfs:label>terraform_labels</rdfs:label>
    <rdfs:comment>The combination of labels configured directly on the resource
 and default labels configured on the provider.</rdfs:comment>
    <rdfs:domain rdf:resource="http://example.org/onto/class/google_kms_crypto_key"/>
    <rdfs:range rdf:resource="http://www.w3.org/2001/XMLSchema#string"/>
  </owl:DatatypeProperty>
  <owl:DatatypeProperty rdf:about="http://example.org/onto/prop/google_kms_crypto_key_create">
    <rdfs:label>create</rdfs:label>
    <rdfs:domain rdf:resource="http://example.org/onto/class/google_kms_crypto_key"/>
    <rdfs:range rdf:resource="http://www.w3.org/2001/XMLSchema#string"/>
  </owl:DatatypeProperty>
  <owl:DatatypeProperty rdf:about="http://example.org/onto/prop/google_kms_crypto_key_delete">
    <rdfs:label>delete</rdfs:label>
    <rdfs:domain rdf:resource="http://example.org/onto/class/google_kms_crypto_key"/>
    <rdfs:range rdf:resource="http://www.w3.org/2001/XMLSchema#string"/>
  </owl:DatatypeProperty>
  <owl:DatatypeProperty rdf:about="http://example.org/onto/prop/google_kms_crypto_key_update">
    <rdfs:label>update</rdfs:label>
    <rdfs:domain rdf:resource="http://example.org/onto/class/google_kms_crypto_key"/>
    <rdfs:range rdf:resource="http://www.w3.org/2001/XMLSchema#string"/>
  </owl:DatatypeProperty>
  <owl:DatatypeProperty rdf:about="http://example.org/onto/prop/google_kms_crypto_key_algorithm">
    <rdfs:label>algorithm</rdfs:label>
    <rdfs:comment>The algorithm to use when creating a version based on this template.
See the [algorithm reference](https://cloud.google.com/kms/docs/reference/rest/v1/CryptoKeyVersionAlgorithm) for possible inputs.</rdfs:comment>
    <rdfs:domain rdf:resource="http://example.org/onto/class/google_kms_crypto_key"/>
    <rdfs:range rdf:resource="http://www.w3.org/2001/XMLSchema#string"/>
  </owl:DatatypeProperty>
  <owl:DatatypeProperty rdf:about="http://example.org/onto/prop/google_kms_crypto_key_protection_level">
    <rdfs:label>protection_level</rdfs:label>
    <rdfs:comment>The protection level to use when creating a version based on this template. Possible values include "SOFTWARE", "HSM", "EXTERNAL", "EXTERNAL_VPC". Defaults to "SOFTWARE".</rdfs:comment>
    <rdfs:domain rdf:resource="http://example.org/onto/class/google_kms_crypto_key"/>
    <rdfs:range rdf:resource="http://www.w3.org/2001/XMLSchema#string"/>
  </owl:DatatypeProperty>
</rdf:RDF>
