<?xml version="1.0" encoding="UTF-8"?>
<rdf:RDF
  xmlns:rdf="http://www.w3.org/1999/02/22-rdf-syntax-ns#"
  xmlns:rdfs="http://www.w3.org/2000/01/rdf-schema#"
  xmlns:owl="http://www.w3.org/2002/07/owl#"
  xmlns:xsd="http://www.w3.org/2001/XMLSchema#"
  xml:base="http://example.org/onto/">
  <owl:Class rdf:about="http://example.org/onto/class/google_dataproc_batch">
    <rdfs:label>google_dataproc_batch</rdfs:label>
    <rdfs:comment>#
#     ***     AUTO GENERATED CODE    ***    Type: MMv1     ***
#
# ----------------------------------------------------------------------------
#
#     This code is generated by Magic Modules using the following:
#
#     Configuration: https:#github.com/GoogleCloudPlatform/magic-modules/tree/main/mmv1/products/dataproc/Batch.yaml
#     Template:      https:#github.com/GoogleCloudPlatform/magic-modules/tree/main/mmv1/templates/terraform/resource.html.markdown.tmpl
#
#     DO NOT EDIT this file directly. Any changes made to this file will be
#     overwritten during the next generation cycle.
#
# ----------------------------------------------------------------------------
subcategory: "Dataproc"
description: |-
  Dataproc Serverless Batches lets you run Spark workloads without requiring you to
  provision and manage your own Dataproc cluster.
---</rdfs:comment>
  </owl:Class>
  <owl:DatatypeProperty rdf:about="http://example.org/onto/prop/google_dataproc_batch_batch_id">
    <rdfs:label>batch_id</rdfs:label>
    <rdfs:comment>The ID to use for the batch, which will become the final component of the batch's resource name.
This value must be 4-63 characters. Valid characters are /[a-z][0-9]-/.</rdfs:comment>
    <rdfs:domain rdf:resource="http://example.org/onto/class/google_dataproc_batch"/>
    <rdfs:range rdf:resource="http://www.w3.org/2001/XMLSchema#string"/>
  </owl:DatatypeProperty>
  <owl:DatatypeProperty rdf:about="http://example.org/onto/prop/google_dataproc_batch_create_time">
    <rdfs:label>create_time</rdfs:label>
    <rdfs:comment>The time when the batch was created.</rdfs:comment>
    <rdfs:domain rdf:resource="http://example.org/onto/class/google_dataproc_batch"/>
    <rdfs:range rdf:resource="http://www.w3.org/2001/XMLSchema#string"/>
  </owl:DatatypeProperty>
  <owl:DatatypeProperty rdf:about="http://example.org/onto/prop/google_dataproc_batch_creator">
    <rdfs:label>creator</rdfs:label>
    <rdfs:comment>The email address of the user who created the batch.</rdfs:comment>
    <rdfs:domain rdf:resource="http://example.org/onto/class/google_dataproc_batch"/>
    <rdfs:range rdf:resource="http://www.w3.org/2001/XMLSchema#string"/>
  </owl:DatatypeProperty>
  <owl:DatatypeProperty rdf:about="http://example.org/onto/prop/google_dataproc_batch_effective_labels">
    <rdfs:label>effective_labels</rdfs:label>
    <rdfs:comment>All of labels (key/value pairs) present on the resource in GCP, including the labels configured through Terraform, other clients and services.</rdfs:comment>
    <rdfs:domain rdf:resource="http://example.org/onto/class/google_dataproc_batch"/>
    <rdfs:range rdf:resource="http://www.w3.org/2001/XMLSchema#string"/>
  </owl:DatatypeProperty>
  <owl:DatatypeProperty rdf:about="http://example.org/onto/prop/google_dataproc_batch_id">
    <rdfs:label>id</rdfs:label>
    <rdfs:domain rdf:resource="http://example.org/onto/class/google_dataproc_batch"/>
    <rdfs:range rdf:resource="http://www.w3.org/2001/XMLSchema#string"/>
  </owl:DatatypeProperty>
  <owl:DatatypeProperty rdf:about="http://example.org/onto/prop/google_dataproc_batch_labels">
    <rdfs:label>labels</rdfs:label>
    <rdfs:comment>The labels to associate with this batch.


**Note**: This field is non-authoritative, and will only manage the labels present in your configuration.
Please refer to the field 'effective_labels' for all of the labels present on the resource.</rdfs:comment>
    <rdfs:domain rdf:resource="http://example.org/onto/class/google_dataproc_batch"/>
    <rdfs:range rdf:resource="http://www.w3.org/2001/XMLSchema#string"/>
  </owl:DatatypeProperty>
  <owl:DatatypeProperty rdf:about="http://example.org/onto/prop/google_dataproc_batch_location">
    <rdfs:label>location</rdfs:label>
    <rdfs:comment>The location in which the batch will be created in.</rdfs:comment>
    <rdfs:domain rdf:resource="http://example.org/onto/class/google_dataproc_batch"/>
    <rdfs:range rdf:resource="http://www.w3.org/2001/XMLSchema#string"/>
  </owl:DatatypeProperty>
  <owl:DatatypeProperty rdf:about="http://example.org/onto/prop/google_dataproc_batch_name">
    <rdfs:label>name</rdfs:label>
    <rdfs:comment>The resource name of the batch.</rdfs:comment>
    <rdfs:domain rdf:resource="http://example.org/onto/class/google_dataproc_batch"/>
    <rdfs:range rdf:resource="http://www.w3.org/2001/XMLSchema#string"/>
  </owl:DatatypeProperty>
  <owl:DatatypeProperty rdf:about="http://example.org/onto/prop/google_dataproc_batch_operation">
    <rdfs:label>operation</rdfs:label>
    <rdfs:comment>The resource name of the operation associated with this batch.</rdfs:comment>
    <rdfs:domain rdf:resource="http://example.org/onto/class/google_dataproc_batch"/>
    <rdfs:range rdf:resource="http://www.w3.org/2001/XMLSchema#string"/>
  </owl:DatatypeProperty>
  <owl:DatatypeProperty rdf:about="http://example.org/onto/prop/google_dataproc_batch_project">
    <rdfs:label>project</rdfs:label>
    <rdfs:domain rdf:resource="http://example.org/onto/class/google_dataproc_batch"/>
    <rdfs:range rdf:resource="http://www.w3.org/2001/XMLSchema#string"/>
  </owl:DatatypeProperty>
  <owl:DatatypeProperty rdf:about="http://example.org/onto/prop/google_dataproc_batch_runtime_info">
    <rdfs:label>runtime_info</rdfs:label>
    <rdfs:comment>Runtime information about batch execution.</rdfs:comment>
    <rdfs:domain rdf:resource="http://example.org/onto/class/google_dataproc_batch"/>
    <rdfs:range rdf:resource="http://www.w3.org/2001/XMLSchema#string"/>
  </owl:DatatypeProperty>
  <owl:DatatypeProperty rdf:about="http://example.org/onto/prop/google_dataproc_batch_state">
    <rdfs:label>state</rdfs:label>
    <rdfs:comment>The state of the batch. For possible values, see the [API documentation](https://cloud.google.com/dataproc-serverless/docs/reference/rest/v1/projects.locations.batches#State).</rdfs:comment>
    <rdfs:domain rdf:resource="http://example.org/onto/class/google_dataproc_batch"/>
    <rdfs:range rdf:resource="http://www.w3.org/2001/XMLSchema#string"/>
  </owl:DatatypeProperty>
  <owl:DatatypeProperty rdf:about="http://example.org/onto/prop/google_dataproc_batch_state_history">
    <rdfs:label>state_history</rdfs:label>
    <rdfs:comment>Historical state information for the batch.</rdfs:comment>
    <rdfs:domain rdf:resource="http://example.org/onto/class/google_dataproc_batch"/>
    <rdfs:range rdf:resource="http://www.w3.org/2001/XMLSchema#string"/>
  </owl:DatatypeProperty>
  <owl:DatatypeProperty rdf:about="http://example.org/onto/prop/google_dataproc_batch_state_message">
    <rdfs:label>state_message</rdfs:label>
    <rdfs:comment>Batch state details, such as a failure description if the state is FAILED.</rdfs:comment>
    <rdfs:domain rdf:resource="http://example.org/onto/class/google_dataproc_batch"/>
    <rdfs:range rdf:resource="http://www.w3.org/2001/XMLSchema#string"/>
  </owl:DatatypeProperty>
  <owl:DatatypeProperty rdf:about="http://example.org/onto/prop/google_dataproc_batch_state_time">
    <rdfs:label>state_time</rdfs:label>
    <rdfs:comment>Batch state details, such as a failure description if the state is FAILED.</rdfs:comment>
    <rdfs:domain rdf:resource="http://example.org/onto/class/google_dataproc_batch"/>
    <rdfs:range rdf:resource="http://www.w3.org/2001/XMLSchema#string"/>
  </owl:DatatypeProperty>
  <owl:DatatypeProperty rdf:about="http://example.org/onto/prop/google_dataproc_batch_terraform_labels">
    <rdfs:label>terraform_labels</rdfs:label>
    <rdfs:comment>The combination of labels configured directly on the resource
 and default labels configured on the provider.</rdfs:comment>
    <rdfs:domain rdf:resource="http://example.org/onto/class/google_dataproc_batch"/>
    <rdfs:range rdf:resource="http://www.w3.org/2001/XMLSchema#string"/>
  </owl:DatatypeProperty>
  <owl:DatatypeProperty rdf:about="http://example.org/onto/prop/google_dataproc_batch_uuid">
    <rdfs:label>uuid</rdfs:label>
    <rdfs:comment>A batch UUID (Unique Universal Identifier). The service generates this value when it creates the batch.</rdfs:comment>
    <rdfs:domain rdf:resource="http://example.org/onto/class/google_dataproc_batch"/>
    <rdfs:range rdf:resource="http://www.w3.org/2001/XMLSchema#string"/>
  </owl:DatatypeProperty>
  <owl:DatatypeProperty rdf:about="http://example.org/onto/prop/google_dataproc_batch_kms_key">
    <rdfs:label>kms_key</rdfs:label>
    <rdfs:comment>The Cloud KMS key to use for encryption.</rdfs:comment>
    <rdfs:domain rdf:resource="http://example.org/onto/class/google_dataproc_batch"/>
    <rdfs:range rdf:resource="http://www.w3.org/2001/XMLSchema#string"/>
  </owl:DatatypeProperty>
  <owl:DatatypeProperty rdf:about="http://example.org/onto/prop/google_dataproc_batch_network_tags">
    <rdfs:label>network_tags</rdfs:label>
    <rdfs:comment>Tags used for network traffic control.</rdfs:comment>
    <rdfs:domain rdf:resource="http://example.org/onto/class/google_dataproc_batch"/>
    <rdfs:range rdf:resource="http://www.w3.org/2001/XMLSchema#string"/>
  </owl:DatatypeProperty>
  <owl:DatatypeProperty rdf:about="http://example.org/onto/prop/google_dataproc_batch_network_uri">
    <rdfs:label>network_uri</rdfs:label>
    <rdfs:comment>Network configuration for workload execution.</rdfs:comment>
    <rdfs:domain rdf:resource="http://example.org/onto/class/google_dataproc_batch"/>
    <rdfs:range rdf:resource="http://www.w3.org/2001/XMLSchema#string"/>
  </owl:DatatypeProperty>
  <owl:DatatypeProperty rdf:about="http://example.org/onto/prop/google_dataproc_batch_service_account">
    <rdfs:label>service_account</rdfs:label>
    <rdfs:comment>Service account that used to execute workload.</rdfs:comment>
    <rdfs:domain rdf:resource="http://example.org/onto/class/google_dataproc_batch"/>
    <rdfs:range rdf:resource="http://www.w3.org/2001/XMLSchema#string"/>
  </owl:DatatypeProperty>
  <owl:DatatypeProperty rdf:about="http://example.org/onto/prop/google_dataproc_batch_staging_bucket">
    <rdfs:label>staging_bucket</rdfs:label>
    <rdfs:comment>A Cloud Storage bucket used to stage workload dependencies, config files, and store
workload output and other ephemeral data, such as Spark history files. If you do not specify a staging bucket,
Cloud Dataproc will determine a Cloud Storage location according to the region where your workload is running,
and then create and manage project-level, per-location staging and temporary buckets.
This field requires a Cloud Storage bucket name, not a gs://... URI to a Cloud Storage bucket.</rdfs:comment>
    <rdfs:domain rdf:resource="http://example.org/onto/class/google_dataproc_batch"/>
    <rdfs:range rdf:resource="http://www.w3.org/2001/XMLSchema#string"/>
  </owl:DatatypeProperty>
  <owl:DatatypeProperty rdf:about="http://example.org/onto/prop/google_dataproc_batch_subnetwork_uri">
    <rdfs:label>subnetwork_uri</rdfs:label>
    <rdfs:comment>Subnetwork configuration for workload execution.</rdfs:comment>
    <rdfs:domain rdf:resource="http://example.org/onto/class/google_dataproc_batch"/>
    <rdfs:range rdf:resource="http://www.w3.org/2001/XMLSchema#string"/>
  </owl:DatatypeProperty>
  <owl:DatatypeProperty rdf:about="http://example.org/onto/prop/google_dataproc_batch_ttl">
    <rdfs:label>ttl</rdfs:label>
    <rdfs:comment>The duration after which the workload will be terminated.
When the workload exceeds this duration, it will be unconditionally terminated without waiting for ongoing
work to finish. If ttl is not specified for a batch workload, the workload will be allowed to run until it
exits naturally (or run forever without exiting). If ttl is not specified for an interactive session,
it defaults to 24 hours. If ttl is not specified for a batch that uses 2.1+ runtime version, it defaults to 4 hours.
Minimum value is 10 minutes; maximum value is 14 days. If both ttl and idleTtl are specified (for an interactive session),
the conditions are treated as OR conditions: the workload will be terminated when it has been idle for idleTtl or
when ttl has been exceeded, whichever occurs first.</rdfs:comment>
    <rdfs:domain rdf:resource="http://example.org/onto/class/google_dataproc_batch"/>
    <rdfs:range rdf:resource="http://www.w3.org/2001/XMLSchema#string"/>
  </owl:DatatypeProperty>
  <owl:DatatypeProperty rdf:about="http://example.org/onto/prop/google_dataproc_batch_user_workload_authentication_type">
    <rdfs:label>user_workload_authentication_type</rdfs:label>
    <rdfs:comment>Authentication type for the user workload running in containers. Possible values: ["SERVICE_ACCOUNT", "END_USER_CREDENTIALS"]</rdfs:comment>
    <rdfs:domain rdf:resource="http://example.org/onto/class/google_dataproc_batch"/>
    <rdfs:range rdf:resource="http://www.w3.org/2001/XMLSchema#string"/>
  </owl:DatatypeProperty>
  <owl:DatatypeProperty rdf:about="http://example.org/onto/prop/google_dataproc_batch_metastore_service">
    <rdfs:label>metastore_service</rdfs:label>
    <rdfs:comment>Resource name of an existing Dataproc Metastore service.</rdfs:comment>
    <rdfs:domain rdf:resource="http://example.org/onto/class/google_dataproc_batch"/>
    <rdfs:range rdf:resource="http://www.w3.org/2001/XMLSchema#string"/>
  </owl:DatatypeProperty>
  <owl:DatatypeProperty rdf:about="http://example.org/onto/prop/google_dataproc_batch_dataproc_cluster">
    <rdfs:label>dataproc_cluster</rdfs:label>
    <rdfs:comment>Resource name of an existing Dataproc Cluster to act as a Spark History Server for the workload.</rdfs:comment>
    <rdfs:domain rdf:resource="http://example.org/onto/class/google_dataproc_batch"/>
    <rdfs:range rdf:resource="http://www.w3.org/2001/XMLSchema#string"/>
  </owl:DatatypeProperty>
  <owl:DatatypeProperty rdf:about="http://example.org/onto/prop/google_dataproc_batch_archive_uris">
    <rdfs:label>archive_uris</rdfs:label>
    <rdfs:comment>HCFS URIs of archives to be extracted into the working directory of each executor.
Supported file types: .jar, .tar, .tar.gz, .tgz, and .zip.</rdfs:comment>
    <rdfs:domain rdf:resource="http://example.org/onto/class/google_dataproc_batch"/>
    <rdfs:range rdf:resource="http://www.w3.org/2001/XMLSchema#string"/>
  </owl:DatatypeProperty>
  <owl:DatatypeProperty rdf:about="http://example.org/onto/prop/google_dataproc_batch_args">
    <rdfs:label>args</rdfs:label>
    <rdfs:comment>The arguments to pass to the driver. Do not include arguments that can be set as batch
properties, such as --conf, since a collision can occur that causes an incorrect batch submission.</rdfs:comment>
    <rdfs:domain rdf:resource="http://example.org/onto/class/google_dataproc_batch"/>
    <rdfs:range rdf:resource="http://www.w3.org/2001/XMLSchema#string"/>
  </owl:DatatypeProperty>
  <owl:DatatypeProperty rdf:about="http://example.org/onto/prop/google_dataproc_batch_file_uris">
    <rdfs:label>file_uris</rdfs:label>
    <rdfs:comment>HCFS URIs of files to be placed in the working directory of each executor.</rdfs:comment>
    <rdfs:domain rdf:resource="http://example.org/onto/class/google_dataproc_batch"/>
    <rdfs:range rdf:resource="http://www.w3.org/2001/XMLSchema#string"/>
  </owl:DatatypeProperty>
  <owl:DatatypeProperty rdf:about="http://example.org/onto/prop/google_dataproc_batch_jar_file_uris">
    <rdfs:label>jar_file_uris</rdfs:label>
    <rdfs:comment>HCFS URIs of jar files to add to the classpath of the Spark driver and tasks.</rdfs:comment>
    <rdfs:domain rdf:resource="http://example.org/onto/class/google_dataproc_batch"/>
    <rdfs:range rdf:resource="http://www.w3.org/2001/XMLSchema#string"/>
  </owl:DatatypeProperty>
  <owl:DatatypeProperty rdf:about="http://example.org/onto/prop/google_dataproc_batch_main_python_file_uri">
    <rdfs:label>main_python_file_uri</rdfs:label>
    <rdfs:comment>The HCFS URI of the main Python file to use as the Spark driver. Must be a .py file.</rdfs:comment>
    <rdfs:domain rdf:resource="http://example.org/onto/class/google_dataproc_batch"/>
    <rdfs:range rdf:resource="http://www.w3.org/2001/XMLSchema#string"/>
  </owl:DatatypeProperty>
  <owl:DatatypeProperty rdf:about="http://example.org/onto/prop/google_dataproc_batch_python_file_uris">
    <rdfs:label>python_file_uris</rdfs:label>
    <rdfs:comment>HCFS file URIs of Python files to pass to the PySpark framework.
Supported file types: .py, .egg, and .zip.</rdfs:comment>
    <rdfs:domain rdf:resource="http://example.org/onto/class/google_dataproc_batch"/>
    <rdfs:range rdf:resource="http://www.w3.org/2001/XMLSchema#string"/>
  </owl:DatatypeProperty>
  <owl:DatatypeProperty rdf:about="http://example.org/onto/prop/google_dataproc_batch_cohort">
    <rdfs:label>cohort</rdfs:label>
    <rdfs:comment>Optional. Cohort identifier. Identifies families of the workloads having the same shape, e.g. daily ETL jobs.</rdfs:comment>
    <rdfs:domain rdf:resource="http://example.org/onto/class/google_dataproc_batch"/>
    <rdfs:range rdf:resource="http://www.w3.org/2001/XMLSchema#string"/>
  </owl:DatatypeProperty>
  <owl:DatatypeProperty rdf:about="http://example.org/onto/prop/google_dataproc_batch_container_image">
    <rdfs:label>container_image</rdfs:label>
    <rdfs:comment>Optional custom container image for the job runtime environment. If not specified, a default container image will be used.</rdfs:comment>
    <rdfs:domain rdf:resource="http://example.org/onto/class/google_dataproc_batch"/>
    <rdfs:range rdf:resource="http://www.w3.org/2001/XMLSchema#string"/>
  </owl:DatatypeProperty>
  <owl:DatatypeProperty rdf:about="http://example.org/onto/prop/google_dataproc_batch_effective_properties">
    <rdfs:label>effective_properties</rdfs:label>
    <rdfs:comment>A mapping of property names to values, which are used to configure workload execution.</rdfs:comment>
    <rdfs:domain rdf:resource="http://example.org/onto/class/google_dataproc_batch"/>
    <rdfs:range rdf:resource="http://www.w3.org/2001/XMLSchema#string"/>
  </owl:DatatypeProperty>
  <owl:DatatypeProperty rdf:about="http://example.org/onto/prop/google_dataproc_batch_properties">
    <rdfs:label>properties</rdfs:label>
    <rdfs:comment>A mapping of property names to values, which are used to configure workload execution.</rdfs:comment>
    <rdfs:domain rdf:resource="http://example.org/onto/class/google_dataproc_batch"/>
    <rdfs:range rdf:resource="http://www.w3.org/2001/XMLSchema#string"/>
  </owl:DatatypeProperty>
  <owl:DatatypeProperty rdf:about="http://example.org/onto/prop/google_dataproc_batch_version">
    <rdfs:label>version</rdfs:label>
    <rdfs:comment>Version of the batch runtime.</rdfs:comment>
    <rdfs:domain rdf:resource="http://example.org/onto/class/google_dataproc_batch"/>
    <rdfs:range rdf:resource="http://www.w3.org/2001/XMLSchema#string"/>
  </owl:DatatypeProperty>
  <owl:DatatypeProperty rdf:about="http://example.org/onto/prop/google_dataproc_batch_scenarios">
    <rdfs:label>scenarios</rdfs:label>
    <rdfs:comment>Optional. Scenarios for which tunings are applied. Possible values: ["SCALING", "BROADCAST_HASH_JOIN", "MEMORY"]</rdfs:comment>
    <rdfs:domain rdf:resource="http://example.org/onto/class/google_dataproc_batch"/>
    <rdfs:range rdf:resource="http://www.w3.org/2001/XMLSchema#string"/>
  </owl:DatatypeProperty>
  <owl:DatatypeProperty rdf:about="http://example.org/onto/prop/google_dataproc_batch_archive_uris">
    <rdfs:label>archive_uris</rdfs:label>
    <rdfs:comment>HCFS URIs of archives to be extracted into the working directory of each executor.
Supported file types: .jar, .tar, .tar.gz, .tgz, and .zip.</rdfs:comment>
    <rdfs:domain rdf:resource="http://example.org/onto/class/google_dataproc_batch"/>
    <rdfs:range rdf:resource="http://www.w3.org/2001/XMLSchema#string"/>
  </owl:DatatypeProperty>
  <owl:DatatypeProperty rdf:about="http://example.org/onto/prop/google_dataproc_batch_args">
    <rdfs:label>args</rdfs:label>
    <rdfs:comment>The arguments to pass to the driver. Do not include arguments that can be set as batch
properties, such as --conf, since a collision can occur that causes an incorrect batch submission.</rdfs:comment>
    <rdfs:domain rdf:resource="http://example.org/onto/class/google_dataproc_batch"/>
    <rdfs:range rdf:resource="http://www.w3.org/2001/XMLSchema#string"/>
  </owl:DatatypeProperty>
  <owl:DatatypeProperty rdf:about="http://example.org/onto/prop/google_dataproc_batch_file_uris">
    <rdfs:label>file_uris</rdfs:label>
    <rdfs:comment>HCFS URIs of files to be placed in the working directory of each executor.</rdfs:comment>
    <rdfs:domain rdf:resource="http://example.org/onto/class/google_dataproc_batch"/>
    <rdfs:range rdf:resource="http://www.w3.org/2001/XMLSchema#string"/>
  </owl:DatatypeProperty>
  <owl:DatatypeProperty rdf:about="http://example.org/onto/prop/google_dataproc_batch_jar_file_uris">
    <rdfs:label>jar_file_uris</rdfs:label>
    <rdfs:comment>HCFS URIs of jar files to add to the classpath of the Spark driver and tasks.</rdfs:comment>
    <rdfs:domain rdf:resource="http://example.org/onto/class/google_dataproc_batch"/>
    <rdfs:range rdf:resource="http://www.w3.org/2001/XMLSchema#string"/>
  </owl:DatatypeProperty>
  <owl:DatatypeProperty rdf:about="http://example.org/onto/prop/google_dataproc_batch_main_class">
    <rdfs:label>main_class</rdfs:label>
    <rdfs:comment>The name of the driver main class. The jar file that contains the class must be in the
classpath or specified in jarFileUris.</rdfs:comment>
    <rdfs:domain rdf:resource="http://example.org/onto/class/google_dataproc_batch"/>
    <rdfs:range rdf:resource="http://www.w3.org/2001/XMLSchema#string"/>
  </owl:DatatypeProperty>
  <owl:DatatypeProperty rdf:about="http://example.org/onto/prop/google_dataproc_batch_main_jar_file_uri">
    <rdfs:label>main_jar_file_uri</rdfs:label>
    <rdfs:comment>The HCFS URI of the jar file that contains the main class.</rdfs:comment>
    <rdfs:domain rdf:resource="http://example.org/onto/class/google_dataproc_batch"/>
    <rdfs:range rdf:resource="http://www.w3.org/2001/XMLSchema#string"/>
  </owl:DatatypeProperty>
  <owl:DatatypeProperty rdf:about="http://example.org/onto/prop/google_dataproc_batch_archive_uris">
    <rdfs:label>archive_uris</rdfs:label>
    <rdfs:comment>HCFS URIs of archives to be extracted into the working directory of each executor.
Supported file types: .jar, .tar, .tar.gz, .tgz, and .zip.</rdfs:comment>
    <rdfs:domain rdf:resource="http://example.org/onto/class/google_dataproc_batch"/>
    <rdfs:range rdf:resource="http://www.w3.org/2001/XMLSchema#string"/>
  </owl:DatatypeProperty>
  <owl:DatatypeProperty rdf:about="http://example.org/onto/prop/google_dataproc_batch_args">
    <rdfs:label>args</rdfs:label>
    <rdfs:comment>The arguments to pass to the driver. Do not include arguments that can be set as batch
properties, such as --conf, since a collision can occur that causes an incorrect batch submission.</rdfs:comment>
    <rdfs:domain rdf:resource="http://example.org/onto/class/google_dataproc_batch"/>
    <rdfs:range rdf:resource="http://www.w3.org/2001/XMLSchema#string"/>
  </owl:DatatypeProperty>
  <owl:DatatypeProperty rdf:about="http://example.org/onto/prop/google_dataproc_batch_file_uris">
    <rdfs:label>file_uris</rdfs:label>
    <rdfs:comment>HCFS URIs of files to be placed in the working directory of each executor.</rdfs:comment>
    <rdfs:domain rdf:resource="http://example.org/onto/class/google_dataproc_batch"/>
    <rdfs:range rdf:resource="http://www.w3.org/2001/XMLSchema#string"/>
  </owl:DatatypeProperty>
  <owl:DatatypeProperty rdf:about="http://example.org/onto/prop/google_dataproc_batch_main_r_file_uri">
    <rdfs:label>main_r_file_uri</rdfs:label>
    <rdfs:comment>The HCFS URI of the main R file to use as the driver. Must be a .R or .r file.</rdfs:comment>
    <rdfs:domain rdf:resource="http://example.org/onto/class/google_dataproc_batch"/>
    <rdfs:range rdf:resource="http://www.w3.org/2001/XMLSchema#string"/>
  </owl:DatatypeProperty>
  <owl:DatatypeProperty rdf:about="http://example.org/onto/prop/google_dataproc_batch_jar_file_uris">
    <rdfs:label>jar_file_uris</rdfs:label>
    <rdfs:comment>HCFS URIs of jar files to be added to the Spark CLASSPATH.</rdfs:comment>
    <rdfs:domain rdf:resource="http://example.org/onto/class/google_dataproc_batch"/>
    <rdfs:range rdf:resource="http://www.w3.org/2001/XMLSchema#string"/>
  </owl:DatatypeProperty>
  <owl:DatatypeProperty rdf:about="http://example.org/onto/prop/google_dataproc_batch_query_file_uri">
    <rdfs:label>query_file_uri</rdfs:label>
    <rdfs:comment>The HCFS URI of the script that contains Spark SQL queries to execute.</rdfs:comment>
    <rdfs:domain rdf:resource="http://example.org/onto/class/google_dataproc_batch"/>
    <rdfs:range rdf:resource="http://www.w3.org/2001/XMLSchema#string"/>
  </owl:DatatypeProperty>
  <owl:DatatypeProperty rdf:about="http://example.org/onto/prop/google_dataproc_batch_query_variables">
    <rdfs:label>query_variables</rdfs:label>
    <rdfs:comment>Mapping of query variable names to values (equivalent to the Spark SQL command: SET name="value";).</rdfs:comment>
    <rdfs:domain rdf:resource="http://example.org/onto/class/google_dataproc_batch"/>
    <rdfs:range rdf:resource="http://www.w3.org/2001/XMLSchema#string"/>
  </owl:DatatypeProperty>
  <owl:DatatypeProperty rdf:about="http://example.org/onto/prop/google_dataproc_batch_create">
    <rdfs:label>create</rdfs:label>
    <rdfs:domain rdf:resource="http://example.org/onto/class/google_dataproc_batch"/>
    <rdfs:range rdf:resource="http://www.w3.org/2001/XMLSchema#string"/>
  </owl:DatatypeProperty>
  <owl:DatatypeProperty rdf:about="http://example.org/onto/prop/google_dataproc_batch_delete">
    <rdfs:label>delete</rdfs:label>
    <rdfs:domain rdf:resource="http://example.org/onto/class/google_dataproc_batch"/>
    <rdfs:range rdf:resource="http://www.w3.org/2001/XMLSchema#string"/>
  </owl:DatatypeProperty>
  <owl:DatatypeProperty rdf:about="http://example.org/onto/prop/google_dataproc_batch_update">
    <rdfs:label>update</rdfs:label>
    <rdfs:domain rdf:resource="http://example.org/onto/class/google_dataproc_batch"/>
    <rdfs:range rdf:resource="http://www.w3.org/2001/XMLSchema#string"/>
  </owl:DatatypeProperty>
</rdf:RDF>
