<?xml version="1.0" encoding="UTF-8"?>
<rdf:RDF
  xmlns:rdf="http://www.w3.org/1999/02/22-rdf-syntax-ns#"
  xmlns:rdfs="http://www.w3.org/2000/01/rdf-schema#"
  xmlns:owl="http://www.w3.org/2002/07/owl#"
  xmlns:xsd="http://www.w3.org/2001/XMLSchema#"
  xml:base="http://example.org/onto/">
  <owl:Class rdf:about="http://example.org/onto/class/google_storage_transfer_job">
    <rdfs:label>google_storage_transfer_job</rdfs:label>
    <rdfs:comment>#
#     ***     AUTO GENERATED CODE    ***    Type: Handwritten     ***
#
# ----------------------------------------------------------------------------
#
#     This code is generated by Magic Modules using the following:
#
#     Source file: https://github.com/GoogleCloudPlatform/magic-modules/tree/main/mmv1/third_party/terraform/website/docs/r/storage_transfer_job.html.markdown
#
#     DO NOT EDIT this file directly. Any changes made to this file will be
#     overwritten during the next generation cycle.
#
# ----------------------------------------------------------------------------
subcategory: "Storage Transfer Service"
description: |-
  Creates a new Transfer Job in Google Cloud Storage Transfer.
---</rdfs:comment>
  </owl:Class>
  <owl:DatatypeProperty rdf:about="http://example.org/onto/prop/google_storage_transfer_job_creation_time">
    <rdfs:label>creation_time</rdfs:label>
    <rdfs:comment>When the Transfer Job was created.</rdfs:comment>
    <rdfs:domain rdf:resource="http://example.org/onto/class/google_storage_transfer_job"/>
    <rdfs:range rdf:resource="http://www.w3.org/2001/XMLSchema#string"/>
  </owl:DatatypeProperty>
  <owl:DatatypeProperty rdf:about="http://example.org/onto/prop/google_storage_transfer_job_deletion_time">
    <rdfs:label>deletion_time</rdfs:label>
    <rdfs:comment>When the Transfer Job was deleted.</rdfs:comment>
    <rdfs:domain rdf:resource="http://example.org/onto/class/google_storage_transfer_job"/>
    <rdfs:range rdf:resource="http://www.w3.org/2001/XMLSchema#string"/>
  </owl:DatatypeProperty>
  <owl:DatatypeProperty rdf:about="http://example.org/onto/prop/google_storage_transfer_job_description">
    <rdfs:label>description</rdfs:label>
    <rdfs:comment>Unique description to identify the Transfer Job.</rdfs:comment>
    <rdfs:domain rdf:resource="http://example.org/onto/class/google_storage_transfer_job"/>
    <rdfs:range rdf:resource="http://www.w3.org/2001/XMLSchema#string"/>
  </owl:DatatypeProperty>
  <owl:DatatypeProperty rdf:about="http://example.org/onto/prop/google_storage_transfer_job_id">
    <rdfs:label>id</rdfs:label>
    <rdfs:domain rdf:resource="http://example.org/onto/class/google_storage_transfer_job"/>
    <rdfs:range rdf:resource="http://www.w3.org/2001/XMLSchema#string"/>
  </owl:DatatypeProperty>
  <owl:DatatypeProperty rdf:about="http://example.org/onto/prop/google_storage_transfer_job_last_modification_time">
    <rdfs:label>last_modification_time</rdfs:label>
    <rdfs:comment>When the Transfer Job was last modified.</rdfs:comment>
    <rdfs:domain rdf:resource="http://example.org/onto/class/google_storage_transfer_job"/>
    <rdfs:range rdf:resource="http://www.w3.org/2001/XMLSchema#string"/>
  </owl:DatatypeProperty>
  <owl:DatatypeProperty rdf:about="http://example.org/onto/prop/google_storage_transfer_job_name">
    <rdfs:label>name</rdfs:label>
    <rdfs:comment>The name of the Transfer Job.</rdfs:comment>
    <rdfs:domain rdf:resource="http://example.org/onto/class/google_storage_transfer_job"/>
    <rdfs:range rdf:resource="http://www.w3.org/2001/XMLSchema#string"/>
  </owl:DatatypeProperty>
  <owl:DatatypeProperty rdf:about="http://example.org/onto/prop/google_storage_transfer_job_project">
    <rdfs:label>project</rdfs:label>
    <rdfs:comment>The project in which the resource belongs. If it is not provided, the provider project is used.</rdfs:comment>
    <rdfs:domain rdf:resource="http://example.org/onto/class/google_storage_transfer_job"/>
    <rdfs:range rdf:resource="http://www.w3.org/2001/XMLSchema#string"/>
  </owl:DatatypeProperty>
  <owl:DatatypeProperty rdf:about="http://example.org/onto/prop/google_storage_transfer_job_service_account">
    <rdfs:label>service_account</rdfs:label>
    <rdfs:comment>The user-managed service account to run the job. If this field is specified, the given service account is granted the necessary permissions to all applicable resources (e.g. GCS buckets) required by the job.</rdfs:comment>
    <rdfs:domain rdf:resource="http://example.org/onto/class/google_storage_transfer_job"/>
    <rdfs:range rdf:resource="http://www.w3.org/2001/XMLSchema#string"/>
  </owl:DatatypeProperty>
  <owl:DatatypeProperty rdf:about="http://example.org/onto/prop/google_storage_transfer_job_status">
    <rdfs:label>status</rdfs:label>
    <rdfs:comment>Status of the job. Default: ENABLED. NOTE: The effect of the new job status takes place during a subsequent job run. For example, if you change the job status from ENABLED to DISABLED, and an operation spawned by the transfer is running, the status change would not affect the current operation.</rdfs:comment>
    <rdfs:domain rdf:resource="http://example.org/onto/class/google_storage_transfer_job"/>
    <rdfs:range rdf:resource="http://www.w3.org/2001/XMLSchema#string"/>
  </owl:DatatypeProperty>
  <owl:DatatypeProperty rdf:about="http://example.org/onto/prop/google_storage_transfer_job_event_stream_expiration_time">
    <rdfs:label>event_stream_expiration_time</rdfs:label>
    <rdfs:comment>Specifies the data and time at which Storage Transfer Service stops listening for events from this stream. After this time, any transfers in progress will complete, but no new transfers are initiated</rdfs:comment>
    <rdfs:domain rdf:resource="http://example.org/onto/class/google_storage_transfer_job"/>
    <rdfs:range rdf:resource="http://www.w3.org/2001/XMLSchema#string"/>
  </owl:DatatypeProperty>
  <owl:DatatypeProperty rdf:about="http://example.org/onto/prop/google_storage_transfer_job_event_stream_start_time">
    <rdfs:label>event_stream_start_time</rdfs:label>
    <rdfs:comment>Specifies the date and time that Storage Transfer Service starts listening for events from this stream. If no start time is specified or start time is in the past, Storage Transfer Service starts listening immediately</rdfs:comment>
    <rdfs:domain rdf:resource="http://example.org/onto/class/google_storage_transfer_job"/>
    <rdfs:range rdf:resource="http://www.w3.org/2001/XMLSchema#string"/>
  </owl:DatatypeProperty>
  <owl:DatatypeProperty rdf:about="http://example.org/onto/prop/google_storage_transfer_job_name">
    <rdfs:label>name</rdfs:label>
    <rdfs:comment>Specifies a unique name of the resource such as AWS SQS ARN in the form 'arn:aws:sqs:region:account_id:queue_name', or Pub/Sub subscription resource name in the form 'projects/{project}/subscriptions/{sub}'</rdfs:comment>
    <rdfs:domain rdf:resource="http://example.org/onto/class/google_storage_transfer_job"/>
    <rdfs:range rdf:resource="http://www.w3.org/2001/XMLSchema#string"/>
  </owl:DatatypeProperty>
  <owl:DatatypeProperty rdf:about="http://example.org/onto/prop/google_storage_transfer_job_enable_on_prem_gcs_transfer_logs">
    <rdfs:label>enable_on_prem_gcs_transfer_logs</rdfs:label>
    <rdfs:comment>For transfers with a PosixFilesystem source, this option enables the Cloud Storage transfer logs for this transfer.</rdfs:comment>
    <rdfs:domain rdf:resource="http://example.org/onto/class/google_storage_transfer_job"/>
    <rdfs:range rdf:resource="http://www.w3.org/2001/XMLSchema#string"/>
  </owl:DatatypeProperty>
  <owl:DatatypeProperty rdf:about="http://example.org/onto/prop/google_storage_transfer_job_log_action_states">
    <rdfs:label>log_action_states</rdfs:label>
    <rdfs:comment>States in which logActions are logged. Not supported for transfers with PosifxFilesystem data sources; use enable_on_prem_gcs_transfer_logs instead.</rdfs:comment>
    <rdfs:domain rdf:resource="http://example.org/onto/class/google_storage_transfer_job"/>
    <rdfs:range rdf:resource="http://www.w3.org/2001/XMLSchema#string"/>
  </owl:DatatypeProperty>
  <owl:DatatypeProperty rdf:about="http://example.org/onto/prop/google_storage_transfer_job_log_actions">
    <rdfs:label>log_actions</rdfs:label>
    <rdfs:comment>Specifies the actions to be logged. Not supported for transfers with PosifxFilesystem data sources; use enable_on_prem_gcs_transfer_logs instead.</rdfs:comment>
    <rdfs:domain rdf:resource="http://example.org/onto/class/google_storage_transfer_job"/>
    <rdfs:range rdf:resource="http://www.w3.org/2001/XMLSchema#string"/>
  </owl:DatatypeProperty>
  <owl:DatatypeProperty rdf:about="http://example.org/onto/prop/google_storage_transfer_job_event_types">
    <rdfs:label>event_types</rdfs:label>
    <rdfs:comment>Event types for which a notification is desired. If empty, send notifications for all event types. The valid types are "TRANSFER_OPERATION_SUCCESS", "TRANSFER_OPERATION_FAILED", "TRANSFER_OPERATION_ABORTED".</rdfs:comment>
    <rdfs:domain rdf:resource="http://example.org/onto/class/google_storage_transfer_job"/>
    <rdfs:range rdf:resource="http://www.w3.org/2001/XMLSchema#string"/>
  </owl:DatatypeProperty>
  <owl:DatatypeProperty rdf:about="http://example.org/onto/prop/google_storage_transfer_job_payload_format">
    <rdfs:label>payload_format</rdfs:label>
    <rdfs:comment>The desired format of the notification message payloads. One of "NONE" or "JSON".</rdfs:comment>
    <rdfs:domain rdf:resource="http://example.org/onto/class/google_storage_transfer_job"/>
    <rdfs:range rdf:resource="http://www.w3.org/2001/XMLSchema#string"/>
  </owl:DatatypeProperty>
  <owl:DatatypeProperty rdf:about="http://example.org/onto/prop/google_storage_transfer_job_pubsub_topic">
    <rdfs:label>pubsub_topic</rdfs:label>
    <rdfs:comment>The Topic.name of the Pub/Sub topic to which to publish notifications.</rdfs:comment>
    <rdfs:domain rdf:resource="http://example.org/onto/class/google_storage_transfer_job"/>
    <rdfs:range rdf:resource="http://www.w3.org/2001/XMLSchema#string"/>
  </owl:DatatypeProperty>
  <owl:DatatypeProperty rdf:about="http://example.org/onto/prop/google_storage_transfer_job_bucket_name">
    <rdfs:label>bucket_name</rdfs:label>
    <rdfs:comment>Google Cloud Storage bucket name.</rdfs:comment>
    <rdfs:domain rdf:resource="http://example.org/onto/class/google_storage_transfer_job"/>
    <rdfs:range rdf:resource="http://www.w3.org/2001/XMLSchema#string"/>
  </owl:DatatypeProperty>
  <owl:DatatypeProperty rdf:about="http://example.org/onto/prop/google_storage_transfer_job_path">
    <rdfs:label>path</rdfs:label>
    <rdfs:comment>Google Cloud Storage path in bucket to transfer. Must be an empty string or full path name that ends with a '/'. This field is treated as an object prefix. As such, it should not begin with a '/'.</rdfs:comment>
    <rdfs:domain rdf:resource="http://example.org/onto/class/google_storage_transfer_job"/>
    <rdfs:range rdf:resource="http://www.w3.org/2001/XMLSchema#string"/>
  </owl:DatatypeProperty>
  <owl:DatatypeProperty rdf:about="http://example.org/onto/prop/google_storage_transfer_job_bucket_name">
    <rdfs:label>bucket_name</rdfs:label>
    <rdfs:comment>Google Cloud Storage bucket name.</rdfs:comment>
    <rdfs:domain rdf:resource="http://example.org/onto/class/google_storage_transfer_job"/>
    <rdfs:range rdf:resource="http://www.w3.org/2001/XMLSchema#string"/>
  </owl:DatatypeProperty>
  <owl:DatatypeProperty rdf:about="http://example.org/onto/prop/google_storage_transfer_job_path">
    <rdfs:label>path</rdfs:label>
    <rdfs:comment>Google Cloud Storage path in bucket to transfer. Must be an empty string or full path name that ends with a '/'. This field is treated as an object prefix. As such, it should not begin with a '/'.</rdfs:comment>
    <rdfs:domain rdf:resource="http://example.org/onto/class/google_storage_transfer_job"/>
    <rdfs:range rdf:resource="http://www.w3.org/2001/XMLSchema#string"/>
  </owl:DatatypeProperty>
  <owl:DatatypeProperty rdf:about="http://example.org/onto/prop/google_storage_transfer_job_exclude_prefixes">
    <rdfs:label>exclude_prefixes</rdfs:label>
    <rdfs:comment>exclude_prefixes must follow the requirements described for include_prefixes.</rdfs:comment>
    <rdfs:domain rdf:resource="http://example.org/onto/class/google_storage_transfer_job"/>
    <rdfs:range rdf:resource="http://www.w3.org/2001/XMLSchema#string"/>
  </owl:DatatypeProperty>
  <owl:DatatypeProperty rdf:about="http://example.org/onto/prop/google_storage_transfer_job_include_prefixes">
    <rdfs:label>include_prefixes</rdfs:label>
    <rdfs:comment>If include_refixes is specified, objects that satisfy the object conditions must have names that start with one of the include_prefixes and that do not start with any of the exclude_prefixes. If include_prefixes is not specified, all objects except those that have names starting with one of the exclude_prefixes must satisfy the object conditions.</rdfs:comment>
    <rdfs:domain rdf:resource="http://example.org/onto/class/google_storage_transfer_job"/>
    <rdfs:range rdf:resource="http://www.w3.org/2001/XMLSchema#string"/>
  </owl:DatatypeProperty>
  <owl:DatatypeProperty rdf:about="http://example.org/onto/prop/google_storage_transfer_job_last_modified_before">
    <rdfs:label>last_modified_before</rdfs:label>
    <rdfs:comment>If specified, only objects with a "last modification time" before this timestamp and objects that don't have a "last modification time" are transferred. A timestamp in RFC3339 UTC "Zulu" format, with nanosecond resolution and up to nine fractional digits. Examples: "2014-10-02T15:01:23Z" and "2014-10-02T15:01:23.045123456Z".</rdfs:comment>
    <rdfs:domain rdf:resource="http://example.org/onto/class/google_storage_transfer_job"/>
    <rdfs:range rdf:resource="http://www.w3.org/2001/XMLSchema#string"/>
  </owl:DatatypeProperty>
  <owl:DatatypeProperty rdf:about="http://example.org/onto/prop/google_storage_transfer_job_last_modified_since">
    <rdfs:label>last_modified_since</rdfs:label>
    <rdfs:comment>If specified, only objects with a "last modification time" on or after this timestamp and objects that don't have a "last modification time" are transferred. A timestamp in RFC3339 UTC "Zulu" format, with nanosecond resolution and up to nine fractional digits. Examples: "2014-10-02T15:01:23Z" and "2014-10-02T15:01:23.045123456Z".</rdfs:comment>
    <rdfs:domain rdf:resource="http://example.org/onto/class/google_storage_transfer_job"/>
    <rdfs:range rdf:resource="http://www.w3.org/2001/XMLSchema#string"/>
  </owl:DatatypeProperty>
  <owl:DatatypeProperty rdf:about="http://example.org/onto/prop/google_storage_transfer_job_max_time_elapsed_since_last_modification">
    <rdfs:label>max_time_elapsed_since_last_modification</rdfs:label>
    <rdfs:comment>A duration in seconds with up to nine fractional digits, terminated by 's'. Example: "3.5s".</rdfs:comment>
    <rdfs:domain rdf:resource="http://example.org/onto/class/google_storage_transfer_job"/>
    <rdfs:range rdf:resource="http://www.w3.org/2001/XMLSchema#string"/>
  </owl:DatatypeProperty>
  <owl:DatatypeProperty rdf:about="http://example.org/onto/prop/google_storage_transfer_job_min_time_elapsed_since_last_modification">
    <rdfs:label>min_time_elapsed_since_last_modification</rdfs:label>
    <rdfs:comment>A duration in seconds with up to nine fractional digits, terminated by 's'. Example: "3.5s".</rdfs:comment>
    <rdfs:domain rdf:resource="http://example.org/onto/class/google_storage_transfer_job"/>
    <rdfs:range rdf:resource="http://www.w3.org/2001/XMLSchema#string"/>
  </owl:DatatypeProperty>
  <owl:DatatypeProperty rdf:about="http://example.org/onto/prop/google_storage_transfer_job_delete_objects_from_source_after_transfer">
    <rdfs:label>delete_objects_from_source_after_transfer</rdfs:label>
    <rdfs:comment>Whether objects should be deleted from the source after they are transferred to the sink. Note that this option and delete_objects_unique_in_sink are mutually exclusive.</rdfs:comment>
    <rdfs:domain rdf:resource="http://example.org/onto/class/google_storage_transfer_job"/>
    <rdfs:range rdf:resource="http://www.w3.org/2001/XMLSchema#string"/>
  </owl:DatatypeProperty>
  <owl:DatatypeProperty rdf:about="http://example.org/onto/prop/google_storage_transfer_job_delete_objects_unique_in_sink">
    <rdfs:label>delete_objects_unique_in_sink</rdfs:label>
    <rdfs:comment>Whether objects that exist only in the sink should be deleted. Note that this option and delete_objects_from_source_after_transfer are mutually exclusive.</rdfs:comment>
    <rdfs:domain rdf:resource="http://example.org/onto/class/google_storage_transfer_job"/>
    <rdfs:range rdf:resource="http://www.w3.org/2001/XMLSchema#string"/>
  </owl:DatatypeProperty>
  <owl:DatatypeProperty rdf:about="http://example.org/onto/prop/google_storage_transfer_job_overwrite_objects_already_existing_in_sink">
    <rdfs:label>overwrite_objects_already_existing_in_sink</rdfs:label>
    <rdfs:comment>Whether overwriting objects that already exist in the sink is allowed.</rdfs:comment>
    <rdfs:domain rdf:resource="http://example.org/onto/class/google_storage_transfer_job"/>
    <rdfs:range rdf:resource="http://www.w3.org/2001/XMLSchema#string"/>
  </owl:DatatypeProperty>
  <owl:DatatypeProperty rdf:about="http://example.org/onto/prop/google_storage_transfer_job_overwrite_when">
    <rdfs:label>overwrite_when</rdfs:label>
    <rdfs:comment>When to overwrite objects that already exist in the sink. If not set, overwrite behavior is determined by overwriteObjectsAlreadyExistingInSink.</rdfs:comment>
    <rdfs:domain rdf:resource="http://example.org/onto/class/google_storage_transfer_job"/>
    <rdfs:range rdf:resource="http://www.w3.org/2001/XMLSchema#string"/>
  </owl:DatatypeProperty>
  <owl:DatatypeProperty rdf:about="http://example.org/onto/prop/google_storage_transfer_job_acl">
    <rdfs:label>acl</rdfs:label>
    <rdfs:comment>Specifies how each object's ACLs should be preserved for transfers between Google Cloud Storage buckets</rdfs:comment>
    <rdfs:domain rdf:resource="http://example.org/onto/class/google_storage_transfer_job"/>
    <rdfs:range rdf:resource="http://www.w3.org/2001/XMLSchema#string"/>
  </owl:DatatypeProperty>
  <owl:DatatypeProperty rdf:about="http://example.org/onto/prop/google_storage_transfer_job_gid">
    <rdfs:label>gid</rdfs:label>
    <rdfs:comment>Specifies how each file's POSIX group ID (GID) attribute should be handled by the transfer.</rdfs:comment>
    <rdfs:domain rdf:resource="http://example.org/onto/class/google_storage_transfer_job"/>
    <rdfs:range rdf:resource="http://www.w3.org/2001/XMLSchema#string"/>
  </owl:DatatypeProperty>
  <owl:DatatypeProperty rdf:about="http://example.org/onto/prop/google_storage_transfer_job_kms_key">
    <rdfs:label>kms_key</rdfs:label>
    <rdfs:comment>Specifies how each object's Cloud KMS customer-managed encryption key (CMEK) is preserved for transfers between Google Cloud Storage buckets</rdfs:comment>
    <rdfs:domain rdf:resource="http://example.org/onto/class/google_storage_transfer_job"/>
    <rdfs:range rdf:resource="http://www.w3.org/2001/XMLSchema#string"/>
  </owl:DatatypeProperty>
  <owl:DatatypeProperty rdf:about="http://example.org/onto/prop/google_storage_transfer_job_mode">
    <rdfs:label>mode</rdfs:label>
    <rdfs:comment>Specifies how each file's mode attribute should be handled by the transfer.</rdfs:comment>
    <rdfs:domain rdf:resource="http://example.org/onto/class/google_storage_transfer_job"/>
    <rdfs:range rdf:resource="http://www.w3.org/2001/XMLSchema#string"/>
  </owl:DatatypeProperty>
  <owl:DatatypeProperty rdf:about="http://example.org/onto/prop/google_storage_transfer_job_storage_class">
    <rdfs:label>storage_class</rdfs:label>
    <rdfs:comment>Specifies the storage class to set on objects being transferred to Google Cloud Storage buckets</rdfs:comment>
    <rdfs:domain rdf:resource="http://example.org/onto/class/google_storage_transfer_job"/>
    <rdfs:range rdf:resource="http://www.w3.org/2001/XMLSchema#string"/>
  </owl:DatatypeProperty>
  <owl:DatatypeProperty rdf:about="http://example.org/onto/prop/google_storage_transfer_job_symlink">
    <rdfs:label>symlink</rdfs:label>
    <rdfs:comment>Specifies how symlinks should be handled by the transfer.</rdfs:comment>
    <rdfs:domain rdf:resource="http://example.org/onto/class/google_storage_transfer_job"/>
    <rdfs:range rdf:resource="http://www.w3.org/2001/XMLSchema#string"/>
  </owl:DatatypeProperty>
  <owl:DatatypeProperty rdf:about="http://example.org/onto/prop/google_storage_transfer_job_temporary_hold">
    <rdfs:label>temporary_hold</rdfs:label>
    <rdfs:comment>SSpecifies how each object's temporary hold status should be preserved for transfers between Google Cloud Storage buckets</rdfs:comment>
    <rdfs:domain rdf:resource="http://example.org/onto/class/google_storage_transfer_job"/>
    <rdfs:range rdf:resource="http://www.w3.org/2001/XMLSchema#string"/>
  </owl:DatatypeProperty>
  <owl:DatatypeProperty rdf:about="http://example.org/onto/prop/google_storage_transfer_job_time_created">
    <rdfs:label>time_created</rdfs:label>
    <rdfs:comment>Specifies how each object's timeCreated metadata is preserved for transfers.</rdfs:comment>
    <rdfs:domain rdf:resource="http://example.org/onto/class/google_storage_transfer_job"/>
    <rdfs:range rdf:resource="http://www.w3.org/2001/XMLSchema#string"/>
  </owl:DatatypeProperty>
  <owl:DatatypeProperty rdf:about="http://example.org/onto/prop/google_storage_transfer_job_uid">
    <rdfs:label>uid</rdfs:label>
    <rdfs:comment>Specifies how each file's POSIX user ID (UID) attribute should be handled by the transfer.</rdfs:comment>
    <rdfs:domain rdf:resource="http://example.org/onto/class/google_storage_transfer_job"/>
    <rdfs:range rdf:resource="http://www.w3.org/2001/XMLSchema#string"/>
  </owl:DatatypeProperty>
  <owl:DatatypeProperty rdf:about="http://example.org/onto/prop/google_storage_transfer_job_repeat_interval">
    <rdfs:label>repeat_interval</rdfs:label>
    <rdfs:comment>Interval between the start of each scheduled transfer. If unspecified, the default value is 24 hours. This value may not be less than 1 hour. A duration in seconds with up to nine fractional digits, terminated by 's'. Example: "3.5s".</rdfs:comment>
    <rdfs:domain rdf:resource="http://example.org/onto/class/google_storage_transfer_job"/>
    <rdfs:range rdf:resource="http://www.w3.org/2001/XMLSchema#string"/>
  </owl:DatatypeProperty>
  <owl:DatatypeProperty rdf:about="http://example.org/onto/prop/google_storage_transfer_job_day">
    <rdfs:label>day</rdfs:label>
    <rdfs:comment>Day of month. Must be from 1 to 31 and valid for the year and month.</rdfs:comment>
    <rdfs:domain rdf:resource="http://example.org/onto/class/google_storage_transfer_job"/>
    <rdfs:range rdf:resource="http://www.w3.org/2001/XMLSchema#string"/>
  </owl:DatatypeProperty>
  <owl:DatatypeProperty rdf:about="http://example.org/onto/prop/google_storage_transfer_job_month">
    <rdfs:label>month</rdfs:label>
    <rdfs:comment>Month of year. Must be from 1 to 12.</rdfs:comment>
    <rdfs:domain rdf:resource="http://example.org/onto/class/google_storage_transfer_job"/>
    <rdfs:range rdf:resource="http://www.w3.org/2001/XMLSchema#string"/>
  </owl:DatatypeProperty>
  <owl:DatatypeProperty rdf:about="http://example.org/onto/prop/google_storage_transfer_job_year">
    <rdfs:label>year</rdfs:label>
    <rdfs:comment>Year of date. Must be from 1 to 9999.</rdfs:comment>
    <rdfs:domain rdf:resource="http://example.org/onto/class/google_storage_transfer_job"/>
    <rdfs:range rdf:resource="http://www.w3.org/2001/XMLSchema#string"/>
  </owl:DatatypeProperty>
  <owl:DatatypeProperty rdf:about="http://example.org/onto/prop/google_storage_transfer_job_day">
    <rdfs:label>day</rdfs:label>
    <rdfs:comment>Day of month. Must be from 1 to 31 and valid for the year and month.</rdfs:comment>
    <rdfs:domain rdf:resource="http://example.org/onto/class/google_storage_transfer_job"/>
    <rdfs:range rdf:resource="http://www.w3.org/2001/XMLSchema#string"/>
  </owl:DatatypeProperty>
  <owl:DatatypeProperty rdf:about="http://example.org/onto/prop/google_storage_transfer_job_month">
    <rdfs:label>month</rdfs:label>
    <rdfs:comment>Month of year. Must be from 1 to 12.</rdfs:comment>
    <rdfs:domain rdf:resource="http://example.org/onto/class/google_storage_transfer_job"/>
    <rdfs:range rdf:resource="http://www.w3.org/2001/XMLSchema#string"/>
  </owl:DatatypeProperty>
  <owl:DatatypeProperty rdf:about="http://example.org/onto/prop/google_storage_transfer_job_year">
    <rdfs:label>year</rdfs:label>
    <rdfs:comment>Year of date. Must be from 1 to 9999.</rdfs:comment>
    <rdfs:domain rdf:resource="http://example.org/onto/class/google_storage_transfer_job"/>
    <rdfs:range rdf:resource="http://www.w3.org/2001/XMLSchema#string"/>
  </owl:DatatypeProperty>
  <owl:DatatypeProperty rdf:about="http://example.org/onto/prop/google_storage_transfer_job_hours">
    <rdfs:label>hours</rdfs:label>
    <rdfs:comment>Hours of day in 24 hour format. Should be from 0 to 23.</rdfs:comment>
    <rdfs:domain rdf:resource="http://example.org/onto/class/google_storage_transfer_job"/>
    <rdfs:range rdf:resource="http://www.w3.org/2001/XMLSchema#string"/>
  </owl:DatatypeProperty>
  <owl:DatatypeProperty rdf:about="http://example.org/onto/prop/google_storage_transfer_job_minutes">
    <rdfs:label>minutes</rdfs:label>
    <rdfs:comment>Minutes of hour of day. Must be from 0 to 59.</rdfs:comment>
    <rdfs:domain rdf:resource="http://example.org/onto/class/google_storage_transfer_job"/>
    <rdfs:range rdf:resource="http://www.w3.org/2001/XMLSchema#string"/>
  </owl:DatatypeProperty>
  <owl:DatatypeProperty rdf:about="http://example.org/onto/prop/google_storage_transfer_job_nanos">
    <rdfs:label>nanos</rdfs:label>
    <rdfs:comment>Fractions of seconds in nanoseconds. Must be from 0 to 999,999,999.</rdfs:comment>
    <rdfs:domain rdf:resource="http://example.org/onto/class/google_storage_transfer_job"/>
    <rdfs:range rdf:resource="http://www.w3.org/2001/XMLSchema#string"/>
  </owl:DatatypeProperty>
  <owl:DatatypeProperty rdf:about="http://example.org/onto/prop/google_storage_transfer_job_seconds">
    <rdfs:label>seconds</rdfs:label>
    <rdfs:comment>Seconds of minutes of the time. Must normally be from 0 to 59.</rdfs:comment>
    <rdfs:domain rdf:resource="http://example.org/onto/class/google_storage_transfer_job"/>
    <rdfs:range rdf:resource="http://www.w3.org/2001/XMLSchema#string"/>
  </owl:DatatypeProperty>
  <owl:DatatypeProperty rdf:about="http://example.org/onto/prop/google_storage_transfer_job_sink_agent_pool_name">
    <rdfs:label>sink_agent_pool_name</rdfs:label>
    <rdfs:comment>Specifies the agent pool name associated with the posix data source. When unspecified, the default name is used.</rdfs:comment>
    <rdfs:domain rdf:resource="http://example.org/onto/class/google_storage_transfer_job"/>
    <rdfs:range rdf:resource="http://www.w3.org/2001/XMLSchema#string"/>
  </owl:DatatypeProperty>
  <owl:DatatypeProperty rdf:about="http://example.org/onto/prop/google_storage_transfer_job_source_agent_pool_name">
    <rdfs:label>source_agent_pool_name</rdfs:label>
    <rdfs:comment>Specifies the agent pool name associated with the posix data source. When unspecified, the default name is used.</rdfs:comment>
    <rdfs:domain rdf:resource="http://example.org/onto/class/google_storage_transfer_job"/>
    <rdfs:range rdf:resource="http://www.w3.org/2001/XMLSchema#string"/>
  </owl:DatatypeProperty>
  <owl:DatatypeProperty rdf:about="http://example.org/onto/prop/google_storage_transfer_job_bucket_name">
    <rdfs:label>bucket_name</rdfs:label>
    <rdfs:comment>Name of the bucket.</rdfs:comment>
    <rdfs:domain rdf:resource="http://example.org/onto/class/google_storage_transfer_job"/>
    <rdfs:range rdf:resource="http://www.w3.org/2001/XMLSchema#string"/>
  </owl:DatatypeProperty>
  <owl:DatatypeProperty rdf:about="http://example.org/onto/prop/google_storage_transfer_job_endpoint">
    <rdfs:label>endpoint</rdfs:label>
    <rdfs:comment>Endpoint of the storage service.</rdfs:comment>
    <rdfs:domain rdf:resource="http://example.org/onto/class/google_storage_transfer_job"/>
    <rdfs:range rdf:resource="http://www.w3.org/2001/XMLSchema#string"/>
  </owl:DatatypeProperty>
  <owl:DatatypeProperty rdf:about="http://example.org/onto/prop/google_storage_transfer_job_path">
    <rdfs:label>path</rdfs:label>
    <rdfs:comment>Specifies the path to transfer objects.</rdfs:comment>
    <rdfs:domain rdf:resource="http://example.org/onto/class/google_storage_transfer_job"/>
    <rdfs:range rdf:resource="http://www.w3.org/2001/XMLSchema#string"/>
  </owl:DatatypeProperty>
  <owl:DatatypeProperty rdf:about="http://example.org/onto/prop/google_storage_transfer_job_region">
    <rdfs:label>region</rdfs:label>
    <rdfs:comment>Specifies the region to sign requests with. This can be left blank if requests should be signed with an empty region.</rdfs:comment>
    <rdfs:domain rdf:resource="http://example.org/onto/class/google_storage_transfer_job"/>
    <rdfs:range rdf:resource="http://www.w3.org/2001/XMLSchema#string"/>
  </owl:DatatypeProperty>
  <owl:DatatypeProperty rdf:about="http://example.org/onto/prop/google_storage_transfer_job_auth_method">
    <rdfs:label>auth_method</rdfs:label>
    <rdfs:comment>Authentication and authorization method used by the storage service. When not specified, Transfer Service will attempt to determine right auth method to use.</rdfs:comment>
    <rdfs:domain rdf:resource="http://example.org/onto/class/google_storage_transfer_job"/>
    <rdfs:range rdf:resource="http://www.w3.org/2001/XMLSchema#string"/>
  </owl:DatatypeProperty>
  <owl:DatatypeProperty rdf:about="http://example.org/onto/prop/google_storage_transfer_job_list_api">
    <rdfs:label>list_api</rdfs:label>
    <rdfs:comment>The Listing API to use for discovering objects. When not specified, Transfer Service will attempt to determine the right API to use.</rdfs:comment>
    <rdfs:domain rdf:resource="http://example.org/onto/class/google_storage_transfer_job"/>
    <rdfs:range rdf:resource="http://www.w3.org/2001/XMLSchema#string"/>
  </owl:DatatypeProperty>
  <owl:DatatypeProperty rdf:about="http://example.org/onto/prop/google_storage_transfer_job_protocol">
    <rdfs:label>protocol</rdfs:label>
    <rdfs:comment>The network protocol of the agent. When not specified, the default value of NetworkProtocol NETWORK_PROTOCOL_HTTPS is used.</rdfs:comment>
    <rdfs:domain rdf:resource="http://example.org/onto/class/google_storage_transfer_job"/>
    <rdfs:range rdf:resource="http://www.w3.org/2001/XMLSchema#string"/>
  </owl:DatatypeProperty>
  <owl:DatatypeProperty rdf:about="http://example.org/onto/prop/google_storage_transfer_job_request_model">
    <rdfs:label>request_model</rdfs:label>
    <rdfs:comment>API request model used to call the storage service. When not specified, the default value of RequestModel REQUEST_MODEL_VIRTUAL_HOSTED_STYLE is used.</rdfs:comment>
    <rdfs:domain rdf:resource="http://example.org/onto/class/google_storage_transfer_job"/>
    <rdfs:range rdf:resource="http://www.w3.org/2001/XMLSchema#string"/>
  </owl:DatatypeProperty>
  <owl:DatatypeProperty rdf:about="http://example.org/onto/prop/google_storage_transfer_job_bucket_name">
    <rdfs:label>bucket_name</rdfs:label>
    <rdfs:comment>S3 Bucket name.</rdfs:comment>
    <rdfs:domain rdf:resource="http://example.org/onto/class/google_storage_transfer_job"/>
    <rdfs:range rdf:resource="http://www.w3.org/2001/XMLSchema#string"/>
  </owl:DatatypeProperty>
  <owl:DatatypeProperty rdf:about="http://example.org/onto/prop/google_storage_transfer_job_cloudfront_domain">
    <rdfs:label>cloudfront_domain</rdfs:label>
    <rdfs:comment>The CloudFront distribution domain name pointing to this bucket, to use when fetching. See [Transfer from S3 via CloudFront](https://cloud.google.com/storage-transfer/docs/s3-cloudfront) for more information. Format: https://{id}.cloudfront.net or any valid custom domain. Must begin with https://.</rdfs:comment>
    <rdfs:domain rdf:resource="http://example.org/onto/class/google_storage_transfer_job"/>
    <rdfs:range rdf:resource="http://www.w3.org/2001/XMLSchema#string"/>
  </owl:DatatypeProperty>
  <owl:DatatypeProperty rdf:about="http://example.org/onto/prop/google_storage_transfer_job_credentials_secret">
    <rdfs:label>credentials_secret</rdfs:label>
    <rdfs:comment>The Resource name of a secret in Secret Manager. AWS credentials must be stored in Secret Manager in JSON format. If credentials_secret is specified, do not specify role_arn or aws_access_key. Format: projects/{projectNumber}/secrets/{secret_name}.</rdfs:comment>
    <rdfs:domain rdf:resource="http://example.org/onto/class/google_storage_transfer_job"/>
    <rdfs:range rdf:resource="http://www.w3.org/2001/XMLSchema#string"/>
  </owl:DatatypeProperty>
  <owl:DatatypeProperty rdf:about="http://example.org/onto/prop/google_storage_transfer_job_managed_private_network">
    <rdfs:label>managed_private_network</rdfs:label>
    <rdfs:comment>Egress bytes over a Google-managed private network. This network is shared between other users of Storage Transfer Service.</rdfs:comment>
    <rdfs:domain rdf:resource="http://example.org/onto/class/google_storage_transfer_job"/>
    <rdfs:range rdf:resource="http://www.w3.org/2001/XMLSchema#string"/>
  </owl:DatatypeProperty>
  <owl:DatatypeProperty rdf:about="http://example.org/onto/prop/google_storage_transfer_job_path">
    <rdfs:label>path</rdfs:label>
    <rdfs:comment>S3 Bucket path in bucket to transfer.</rdfs:comment>
    <rdfs:domain rdf:resource="http://example.org/onto/class/google_storage_transfer_job"/>
    <rdfs:range rdf:resource="http://www.w3.org/2001/XMLSchema#string"/>
  </owl:DatatypeProperty>
  <owl:DatatypeProperty rdf:about="http://example.org/onto/prop/google_storage_transfer_job_role_arn">
    <rdfs:label>role_arn</rdfs:label>
    <rdfs:comment>The Amazon Resource Name (ARN) of the role to support temporary credentials via 'AssumeRoleWithWebIdentity'. For more information about ARNs, see [IAM ARNs](https://docs.aws.amazon.com/IAM/latest/UserGuide/reference_identifiers.html#identifiers-arns). When a role ARN is provided, Transfer Service fetches temporary credentials for the session using a 'AssumeRoleWithWebIdentity' call for the provided role using the [GoogleServiceAccount][] for this project.</rdfs:comment>
    <rdfs:domain rdf:resource="http://example.org/onto/class/google_storage_transfer_job"/>
    <rdfs:range rdf:resource="http://www.w3.org/2001/XMLSchema#string"/>
  </owl:DatatypeProperty>
  <owl:DatatypeProperty rdf:about="http://example.org/onto/prop/google_storage_transfer_job_access_key_id">
    <rdfs:label>access_key_id</rdfs:label>
    <rdfs:comment>AWS Key ID.</rdfs:comment>
    <rdfs:domain rdf:resource="http://example.org/onto/class/google_storage_transfer_job"/>
    <rdfs:range rdf:resource="http://www.w3.org/2001/XMLSchema#string"/>
  </owl:DatatypeProperty>
  <owl:DatatypeProperty rdf:about="http://example.org/onto/prop/google_storage_transfer_job_secret_access_key">
    <rdfs:label>secret_access_key</rdfs:label>
    <rdfs:comment>AWS Secret Access Key.</rdfs:comment>
    <rdfs:domain rdf:resource="http://example.org/onto/class/google_storage_transfer_job"/>
    <rdfs:range rdf:resource="http://www.w3.org/2001/XMLSchema#string"/>
  </owl:DatatypeProperty>
  <owl:DatatypeProperty rdf:about="http://example.org/onto/prop/google_storage_transfer_job_container">
    <rdfs:label>container</rdfs:label>
    <rdfs:comment>The container to transfer from the Azure Storage account.</rdfs:comment>
    <rdfs:domain rdf:resource="http://example.org/onto/class/google_storage_transfer_job"/>
    <rdfs:range rdf:resource="http://www.w3.org/2001/XMLSchema#string"/>
  </owl:DatatypeProperty>
  <owl:DatatypeProperty rdf:about="http://example.org/onto/prop/google_storage_transfer_job_credentials_secret">
    <rdfs:label>credentials_secret</rdfs:label>
    <rdfs:comment>The Resource name of a secret in Secret Manager containing SAS Credentials in JSON form. Service Agent must have permissions to access secret. If credentials_secret is specified, do not specify azure_credentials.</rdfs:comment>
    <rdfs:domain rdf:resource="http://example.org/onto/class/google_storage_transfer_job"/>
    <rdfs:range rdf:resource="http://www.w3.org/2001/XMLSchema#string"/>
  </owl:DatatypeProperty>
  <owl:DatatypeProperty rdf:about="http://example.org/onto/prop/google_storage_transfer_job_path">
    <rdfs:label>path</rdfs:label>
    <rdfs:comment>Root path to transfer objects. Must be an empty string or full path name that ends with a '/'. This field is treated as an object prefix. As such, it should generally not begin with a '/'.</rdfs:comment>
    <rdfs:domain rdf:resource="http://example.org/onto/class/google_storage_transfer_job"/>
    <rdfs:range rdf:resource="http://www.w3.org/2001/XMLSchema#string"/>
  </owl:DatatypeProperty>
  <owl:DatatypeProperty rdf:about="http://example.org/onto/prop/google_storage_transfer_job_storage_account">
    <rdfs:label>storage_account</rdfs:label>
    <rdfs:comment>The name of the Azure Storage account.</rdfs:comment>
    <rdfs:domain rdf:resource="http://example.org/onto/class/google_storage_transfer_job"/>
    <rdfs:range rdf:resource="http://www.w3.org/2001/XMLSchema#string"/>
  </owl:DatatypeProperty>
  <owl:DatatypeProperty rdf:about="http://example.org/onto/prop/google_storage_transfer_job_sas_token">
    <rdfs:label>sas_token</rdfs:label>
    <rdfs:comment>Azure shared access signature.</rdfs:comment>
    <rdfs:domain rdf:resource="http://example.org/onto/class/google_storage_transfer_job"/>
    <rdfs:range rdf:resource="http://www.w3.org/2001/XMLSchema#string"/>
  </owl:DatatypeProperty>
  <owl:DatatypeProperty rdf:about="http://example.org/onto/prop/google_storage_transfer_job_client_id">
    <rdfs:label>client_id</rdfs:label>
    <rdfs:comment>The client (application) ID of the application with federated credentials.</rdfs:comment>
    <rdfs:domain rdf:resource="http://example.org/onto/class/google_storage_transfer_job"/>
    <rdfs:range rdf:resource="http://www.w3.org/2001/XMLSchema#string"/>
  </owl:DatatypeProperty>
  <owl:DatatypeProperty rdf:about="http://example.org/onto/prop/google_storage_transfer_job_tenant_id">
    <rdfs:label>tenant_id</rdfs:label>
    <rdfs:comment>The tenant (directory) ID of the application with federated credentials.</rdfs:comment>
    <rdfs:domain rdf:resource="http://example.org/onto/class/google_storage_transfer_job"/>
    <rdfs:range rdf:resource="http://www.w3.org/2001/XMLSchema#string"/>
  </owl:DatatypeProperty>
  <owl:DatatypeProperty rdf:about="http://example.org/onto/prop/google_storage_transfer_job_bucket_name">
    <rdfs:label>bucket_name</rdfs:label>
    <rdfs:comment>Google Cloud Storage bucket name.</rdfs:comment>
    <rdfs:domain rdf:resource="http://example.org/onto/class/google_storage_transfer_job"/>
    <rdfs:range rdf:resource="http://www.w3.org/2001/XMLSchema#string"/>
  </owl:DatatypeProperty>
  <owl:DatatypeProperty rdf:about="http://example.org/onto/prop/google_storage_transfer_job_path">
    <rdfs:label>path</rdfs:label>
    <rdfs:comment>Google Cloud Storage path in bucket to transfer. Must be an empty string or full path name that ends with a '/'. This field is treated as an object prefix. As such, it should not begin with a '/'.</rdfs:comment>
    <rdfs:domain rdf:resource="http://example.org/onto/class/google_storage_transfer_job"/>
    <rdfs:range rdf:resource="http://www.w3.org/2001/XMLSchema#string"/>
  </owl:DatatypeProperty>
  <owl:DatatypeProperty rdf:about="http://example.org/onto/prop/google_storage_transfer_job_bucket_name">
    <rdfs:label>bucket_name</rdfs:label>
    <rdfs:comment>Google Cloud Storage bucket name.</rdfs:comment>
    <rdfs:domain rdf:resource="http://example.org/onto/class/google_storage_transfer_job"/>
    <rdfs:range rdf:resource="http://www.w3.org/2001/XMLSchema#string"/>
  </owl:DatatypeProperty>
  <owl:DatatypeProperty rdf:about="http://example.org/onto/prop/google_storage_transfer_job_path">
    <rdfs:label>path</rdfs:label>
    <rdfs:comment>Google Cloud Storage path in bucket to transfer. Must be an empty string or full path name that ends with a '/'. This field is treated as an object prefix. As such, it should not begin with a '/'.</rdfs:comment>
    <rdfs:domain rdf:resource="http://example.org/onto/class/google_storage_transfer_job"/>
    <rdfs:range rdf:resource="http://www.w3.org/2001/XMLSchema#string"/>
  </owl:DatatypeProperty>
  <owl:DatatypeProperty rdf:about="http://example.org/onto/prop/google_storage_transfer_job_path">
    <rdfs:label>path</rdfs:label>
    <rdfs:comment>Directory path to the filesystem.</rdfs:comment>
    <rdfs:domain rdf:resource="http://example.org/onto/class/google_storage_transfer_job"/>
    <rdfs:range rdf:resource="http://www.w3.org/2001/XMLSchema#string"/>
  </owl:DatatypeProperty>
  <owl:DatatypeProperty rdf:about="http://example.org/onto/prop/google_storage_transfer_job_list_url">
    <rdfs:label>list_url</rdfs:label>
    <rdfs:comment>The URL that points to the file that stores the object list entries. This file must allow public access. Currently, only URLs with HTTP and HTTPS schemes are supported.</rdfs:comment>
    <rdfs:domain rdf:resource="http://example.org/onto/class/google_storage_transfer_job"/>
    <rdfs:range rdf:resource="http://www.w3.org/2001/XMLSchema#string"/>
  </owl:DatatypeProperty>
  <owl:DatatypeProperty rdf:about="http://example.org/onto/prop/google_storage_transfer_job_exclude_prefixes">
    <rdfs:label>exclude_prefixes</rdfs:label>
    <rdfs:comment>exclude_prefixes must follow the requirements described for include_prefixes.</rdfs:comment>
    <rdfs:domain rdf:resource="http://example.org/onto/class/google_storage_transfer_job"/>
    <rdfs:range rdf:resource="http://www.w3.org/2001/XMLSchema#string"/>
  </owl:DatatypeProperty>
  <owl:DatatypeProperty rdf:about="http://example.org/onto/prop/google_storage_transfer_job_include_prefixes">
    <rdfs:label>include_prefixes</rdfs:label>
    <rdfs:comment>If include_refixes is specified, objects that satisfy the object conditions must have names that start with one of the include_prefixes and that do not start with any of the exclude_prefixes. If include_prefixes is not specified, all objects except those that have names starting with one of the exclude_prefixes must satisfy the object conditions.</rdfs:comment>
    <rdfs:domain rdf:resource="http://example.org/onto/class/google_storage_transfer_job"/>
    <rdfs:range rdf:resource="http://www.w3.org/2001/XMLSchema#string"/>
  </owl:DatatypeProperty>
  <owl:DatatypeProperty rdf:about="http://example.org/onto/prop/google_storage_transfer_job_last_modified_before">
    <rdfs:label>last_modified_before</rdfs:label>
    <rdfs:comment>If specified, only objects with a "last modification time" before this timestamp and objects that don't have a "last modification time" are transferred. A timestamp in RFC3339 UTC "Zulu" format, with nanosecond resolution and up to nine fractional digits. Examples: "2014-10-02T15:01:23Z" and "2014-10-02T15:01:23.045123456Z".</rdfs:comment>
    <rdfs:domain rdf:resource="http://example.org/onto/class/google_storage_transfer_job"/>
    <rdfs:range rdf:resource="http://www.w3.org/2001/XMLSchema#string"/>
  </owl:DatatypeProperty>
  <owl:DatatypeProperty rdf:about="http://example.org/onto/prop/google_storage_transfer_job_last_modified_since">
    <rdfs:label>last_modified_since</rdfs:label>
    <rdfs:comment>If specified, only objects with a "last modification time" on or after this timestamp and objects that don't have a "last modification time" are transferred. A timestamp in RFC3339 UTC "Zulu" format, with nanosecond resolution and up to nine fractional digits. Examples: "2014-10-02T15:01:23Z" and "2014-10-02T15:01:23.045123456Z".</rdfs:comment>
    <rdfs:domain rdf:resource="http://example.org/onto/class/google_storage_transfer_job"/>
    <rdfs:range rdf:resource="http://www.w3.org/2001/XMLSchema#string"/>
  </owl:DatatypeProperty>
  <owl:DatatypeProperty rdf:about="http://example.org/onto/prop/google_storage_transfer_job_max_time_elapsed_since_last_modification">
    <rdfs:label>max_time_elapsed_since_last_modification</rdfs:label>
    <rdfs:comment>A duration in seconds with up to nine fractional digits, terminated by 's'. Example: "3.5s".</rdfs:comment>
    <rdfs:domain rdf:resource="http://example.org/onto/class/google_storage_transfer_job"/>
    <rdfs:range rdf:resource="http://www.w3.org/2001/XMLSchema#string"/>
  </owl:DatatypeProperty>
  <owl:DatatypeProperty rdf:about="http://example.org/onto/prop/google_storage_transfer_job_min_time_elapsed_since_last_modification">
    <rdfs:label>min_time_elapsed_since_last_modification</rdfs:label>
    <rdfs:comment>A duration in seconds with up to nine fractional digits, terminated by 's'. Example: "3.5s".</rdfs:comment>
    <rdfs:domain rdf:resource="http://example.org/onto/class/google_storage_transfer_job"/>
    <rdfs:range rdf:resource="http://www.w3.org/2001/XMLSchema#string"/>
  </owl:DatatypeProperty>
  <owl:DatatypeProperty rdf:about="http://example.org/onto/prop/google_storage_transfer_job_root_directory">
    <rdfs:label>root_directory</rdfs:label>
    <rdfs:comment>Root directory path to the filesystem.</rdfs:comment>
    <rdfs:domain rdf:resource="http://example.org/onto/class/google_storage_transfer_job"/>
    <rdfs:range rdf:resource="http://www.w3.org/2001/XMLSchema#string"/>
  </owl:DatatypeProperty>
  <owl:DatatypeProperty rdf:about="http://example.org/onto/prop/google_storage_transfer_job_root_directory">
    <rdfs:label>root_directory</rdfs:label>
    <rdfs:comment>Root directory path to the filesystem.</rdfs:comment>
    <rdfs:domain rdf:resource="http://example.org/onto/class/google_storage_transfer_job"/>
    <rdfs:range rdf:resource="http://www.w3.org/2001/XMLSchema#string"/>
  </owl:DatatypeProperty>
  <owl:DatatypeProperty rdf:about="http://example.org/onto/prop/google_storage_transfer_job_delete_objects_from_source_after_transfer">
    <rdfs:label>delete_objects_from_source_after_transfer</rdfs:label>
    <rdfs:comment>Whether objects should be deleted from the source after they are transferred to the sink. Note that this option and delete_objects_unique_in_sink are mutually exclusive.</rdfs:comment>
    <rdfs:domain rdf:resource="http://example.org/onto/class/google_storage_transfer_job"/>
    <rdfs:range rdf:resource="http://www.w3.org/2001/XMLSchema#string"/>
  </owl:DatatypeProperty>
  <owl:DatatypeProperty rdf:about="http://example.org/onto/prop/google_storage_transfer_job_delete_objects_unique_in_sink">
    <rdfs:label>delete_objects_unique_in_sink</rdfs:label>
    <rdfs:comment>Whether objects that exist only in the sink should be deleted. Note that this option and delete_objects_from_source_after_transfer are mutually exclusive.</rdfs:comment>
    <rdfs:domain rdf:resource="http://example.org/onto/class/google_storage_transfer_job"/>
    <rdfs:range rdf:resource="http://www.w3.org/2001/XMLSchema#string"/>
  </owl:DatatypeProperty>
  <owl:DatatypeProperty rdf:about="http://example.org/onto/prop/google_storage_transfer_job_overwrite_objects_already_existing_in_sink">
    <rdfs:label>overwrite_objects_already_existing_in_sink</rdfs:label>
    <rdfs:comment>Whether overwriting objects that already exist in the sink is allowed.</rdfs:comment>
    <rdfs:domain rdf:resource="http://example.org/onto/class/google_storage_transfer_job"/>
    <rdfs:range rdf:resource="http://www.w3.org/2001/XMLSchema#string"/>
  </owl:DatatypeProperty>
  <owl:DatatypeProperty rdf:about="http://example.org/onto/prop/google_storage_transfer_job_overwrite_when">
    <rdfs:label>overwrite_when</rdfs:label>
    <rdfs:comment>When to overwrite objects that already exist in the sink. If not set, overwrite behavior is determined by overwriteObjectsAlreadyExistingInSink.</rdfs:comment>
    <rdfs:domain rdf:resource="http://example.org/onto/class/google_storage_transfer_job"/>
    <rdfs:range rdf:resource="http://www.w3.org/2001/XMLSchema#string"/>
  </owl:DatatypeProperty>
  <owl:DatatypeProperty rdf:about="http://example.org/onto/prop/google_storage_transfer_job_acl">
    <rdfs:label>acl</rdfs:label>
    <rdfs:comment>Specifies how each object's ACLs should be preserved for transfers between Google Cloud Storage buckets</rdfs:comment>
    <rdfs:domain rdf:resource="http://example.org/onto/class/google_storage_transfer_job"/>
    <rdfs:range rdf:resource="http://www.w3.org/2001/XMLSchema#string"/>
  </owl:DatatypeProperty>
  <owl:DatatypeProperty rdf:about="http://example.org/onto/prop/google_storage_transfer_job_gid">
    <rdfs:label>gid</rdfs:label>
    <rdfs:comment>Specifies how each file's POSIX group ID (GID) attribute should be handled by the transfer.</rdfs:comment>
    <rdfs:domain rdf:resource="http://example.org/onto/class/google_storage_transfer_job"/>
    <rdfs:range rdf:resource="http://www.w3.org/2001/XMLSchema#string"/>
  </owl:DatatypeProperty>
  <owl:DatatypeProperty rdf:about="http://example.org/onto/prop/google_storage_transfer_job_kms_key">
    <rdfs:label>kms_key</rdfs:label>
    <rdfs:comment>Specifies how each object's Cloud KMS customer-managed encryption key (CMEK) is preserved for transfers between Google Cloud Storage buckets</rdfs:comment>
    <rdfs:domain rdf:resource="http://example.org/onto/class/google_storage_transfer_job"/>
    <rdfs:range rdf:resource="http://www.w3.org/2001/XMLSchema#string"/>
  </owl:DatatypeProperty>
  <owl:DatatypeProperty rdf:about="http://example.org/onto/prop/google_storage_transfer_job_mode">
    <rdfs:label>mode</rdfs:label>
    <rdfs:comment>Specifies how each file's mode attribute should be handled by the transfer.</rdfs:comment>
    <rdfs:domain rdf:resource="http://example.org/onto/class/google_storage_transfer_job"/>
    <rdfs:range rdf:resource="http://www.w3.org/2001/XMLSchema#string"/>
  </owl:DatatypeProperty>
  <owl:DatatypeProperty rdf:about="http://example.org/onto/prop/google_storage_transfer_job_storage_class">
    <rdfs:label>storage_class</rdfs:label>
    <rdfs:comment>Specifies the storage class to set on objects being transferred to Google Cloud Storage buckets</rdfs:comment>
    <rdfs:domain rdf:resource="http://example.org/onto/class/google_storage_transfer_job"/>
    <rdfs:range rdf:resource="http://www.w3.org/2001/XMLSchema#string"/>
  </owl:DatatypeProperty>
  <owl:DatatypeProperty rdf:about="http://example.org/onto/prop/google_storage_transfer_job_symlink">
    <rdfs:label>symlink</rdfs:label>
    <rdfs:comment>Specifies how symlinks should be handled by the transfer.</rdfs:comment>
    <rdfs:domain rdf:resource="http://example.org/onto/class/google_storage_transfer_job"/>
    <rdfs:range rdf:resource="http://www.w3.org/2001/XMLSchema#string"/>
  </owl:DatatypeProperty>
  <owl:DatatypeProperty rdf:about="http://example.org/onto/prop/google_storage_transfer_job_temporary_hold">
    <rdfs:label>temporary_hold</rdfs:label>
    <rdfs:comment>SSpecifies how each object's temporary hold status should be preserved for transfers between Google Cloud Storage buckets</rdfs:comment>
    <rdfs:domain rdf:resource="http://example.org/onto/class/google_storage_transfer_job"/>
    <rdfs:range rdf:resource="http://www.w3.org/2001/XMLSchema#string"/>
  </owl:DatatypeProperty>
  <owl:DatatypeProperty rdf:about="http://example.org/onto/prop/google_storage_transfer_job_time_created">
    <rdfs:label>time_created</rdfs:label>
    <rdfs:comment>Specifies how each object's timeCreated metadata is preserved for transfers.</rdfs:comment>
    <rdfs:domain rdf:resource="http://example.org/onto/class/google_storage_transfer_job"/>
    <rdfs:range rdf:resource="http://www.w3.org/2001/XMLSchema#string"/>
  </owl:DatatypeProperty>
  <owl:DatatypeProperty rdf:about="http://example.org/onto/prop/google_storage_transfer_job_uid">
    <rdfs:label>uid</rdfs:label>
    <rdfs:comment>Specifies how each file's POSIX user ID (UID) attribute should be handled by the transfer.</rdfs:comment>
    <rdfs:domain rdf:resource="http://example.org/onto/class/google_storage_transfer_job"/>
    <rdfs:range rdf:resource="http://www.w3.org/2001/XMLSchema#string"/>
  </owl:DatatypeProperty>
</rdf:RDF>
