<?xml version="1.0" encoding="UTF-8"?>
<rdf:RDF
  xmlns:rdf="http://www.w3.org/1999/02/22-rdf-syntax-ns#"
  xmlns:rdfs="http://www.w3.org/2000/01/rdf-schema#"
  xmlns:owl="http://www.w3.org/2002/07/owl#"
  xmlns:xsd="http://www.w3.org/2001/XMLSchema#"
  xml:base="http://example.org/onto/">
  <owl:Class rdf:about="http://example.org/onto/class/google_bigquery_routine">
    <rdfs:label>google_bigquery_routine</rdfs:label>
    <rdfs:comment>#
#     ***     AUTO GENERATED CODE    ***    Type: MMv1     ***
#
# ----------------------------------------------------------------------------
#
#     This code is generated by Magic Modules using the following:
#
#     Configuration: https:#github.com/GoogleCloudPlatform/magic-modules/tree/main/mmv1/products/bigquery/Routine.yaml
#     Template:      https:#github.com/GoogleCloudPlatform/magic-modules/tree/main/mmv1/templates/terraform/resource.html.markdown.tmpl
#
#     DO NOT EDIT this file directly. Any changes made to this file will be
#     overwritten during the next generation cycle.
#
# ----------------------------------------------------------------------------
subcategory: "BigQuery"
description: |-
  A user-defined function or a stored procedure that belongs to a Dataset
---</rdfs:comment>
  </owl:Class>
  <owl:DatatypeProperty rdf:about="http://example.org/onto/prop/google_bigquery_routine_creation_time">
    <rdfs:label>creation_time</rdfs:label>
    <rdfs:comment>The time when this routine was created, in milliseconds since the
epoch.</rdfs:comment>
    <rdfs:domain rdf:resource="http://example.org/onto/class/google_bigquery_routine"/>
    <rdfs:range rdf:resource="http://www.w3.org/2001/XMLSchema#string"/>
  </owl:DatatypeProperty>
  <owl:DatatypeProperty rdf:about="http://example.org/onto/prop/google_bigquery_routine_data_governance_type">
    <rdfs:label>data_governance_type</rdfs:label>
    <rdfs:comment>If set to DATA_MASKING, the function is validated and made available as a masking function. For more information, see https://cloud.google.com/bigquery/docs/user-defined-functions#custom-mask Possible values: ["DATA_MASKING"]</rdfs:comment>
    <rdfs:domain rdf:resource="http://example.org/onto/class/google_bigquery_routine"/>
    <rdfs:range rdf:resource="http://www.w3.org/2001/XMLSchema#string"/>
  </owl:DatatypeProperty>
  <owl:DatatypeProperty rdf:about="http://example.org/onto/prop/google_bigquery_routine_dataset_id">
    <rdfs:label>dataset_id</rdfs:label>
    <rdfs:comment>The ID of the dataset containing this routine</rdfs:comment>
    <rdfs:domain rdf:resource="http://example.org/onto/class/google_bigquery_routine"/>
    <rdfs:range rdf:resource="http://www.w3.org/2001/XMLSchema#string"/>
  </owl:DatatypeProperty>
  <owl:DatatypeProperty rdf:about="http://example.org/onto/prop/google_bigquery_routine_definition_body">
    <rdfs:label>definition_body</rdfs:label>
    <rdfs:comment>The body of the routine. For functions, this is the expression in the AS clause.
If language=SQL, it is the substring inside (but excluding) the parentheses.</rdfs:comment>
    <rdfs:domain rdf:resource="http://example.org/onto/class/google_bigquery_routine"/>
    <rdfs:range rdf:resource="http://www.w3.org/2001/XMLSchema#string"/>
  </owl:DatatypeProperty>
  <owl:DatatypeProperty rdf:about="http://example.org/onto/prop/google_bigquery_routine_description">
    <rdfs:label>description</rdfs:label>
    <rdfs:comment>The description of the routine if defined.</rdfs:comment>
    <rdfs:domain rdf:resource="http://example.org/onto/class/google_bigquery_routine"/>
    <rdfs:range rdf:resource="http://www.w3.org/2001/XMLSchema#string"/>
  </owl:DatatypeProperty>
  <owl:DatatypeProperty rdf:about="http://example.org/onto/prop/google_bigquery_routine_determinism_level">
    <rdfs:label>determinism_level</rdfs:label>
    <rdfs:comment>The determinism level of the JavaScript UDF if defined. Possible values: ["DETERMINISM_LEVEL_UNSPECIFIED", "DETERMINISTIC", "NOT_DETERMINISTIC"]</rdfs:comment>
    <rdfs:domain rdf:resource="http://example.org/onto/class/google_bigquery_routine"/>
    <rdfs:range rdf:resource="http://www.w3.org/2001/XMLSchema#string"/>
  </owl:DatatypeProperty>
  <owl:DatatypeProperty rdf:about="http://example.org/onto/prop/google_bigquery_routine_id">
    <rdfs:label>id</rdfs:label>
    <rdfs:domain rdf:resource="http://example.org/onto/class/google_bigquery_routine"/>
    <rdfs:range rdf:resource="http://www.w3.org/2001/XMLSchema#string"/>
  </owl:DatatypeProperty>
  <owl:DatatypeProperty rdf:about="http://example.org/onto/prop/google_bigquery_routine_imported_libraries">
    <rdfs:label>imported_libraries</rdfs:label>
    <rdfs:comment>Optional. If language = "JAVASCRIPT", this field stores the path of the
imported JAVASCRIPT libraries.</rdfs:comment>
    <rdfs:domain rdf:resource="http://example.org/onto/class/google_bigquery_routine"/>
    <rdfs:range rdf:resource="http://www.w3.org/2001/XMLSchema#string"/>
  </owl:DatatypeProperty>
  <owl:DatatypeProperty rdf:about="http://example.org/onto/prop/google_bigquery_routine_language">
    <rdfs:label>language</rdfs:label>
    <rdfs:comment>The language of the routine. Possible values: ["SQL", "JAVASCRIPT", "PYTHON", "JAVA", "SCALA"]</rdfs:comment>
    <rdfs:domain rdf:resource="http://example.org/onto/class/google_bigquery_routine"/>
    <rdfs:range rdf:resource="http://www.w3.org/2001/XMLSchema#string"/>
  </owl:DatatypeProperty>
  <owl:DatatypeProperty rdf:about="http://example.org/onto/prop/google_bigquery_routine_last_modified_time">
    <rdfs:label>last_modified_time</rdfs:label>
    <rdfs:comment>The time when this routine was modified, in milliseconds since the
epoch.</rdfs:comment>
    <rdfs:domain rdf:resource="http://example.org/onto/class/google_bigquery_routine"/>
    <rdfs:range rdf:resource="http://www.w3.org/2001/XMLSchema#string"/>
  </owl:DatatypeProperty>
  <owl:DatatypeProperty rdf:about="http://example.org/onto/prop/google_bigquery_routine_project">
    <rdfs:label>project</rdfs:label>
    <rdfs:domain rdf:resource="http://example.org/onto/class/google_bigquery_routine"/>
    <rdfs:range rdf:resource="http://www.w3.org/2001/XMLSchema#string"/>
  </owl:DatatypeProperty>
  <owl:DatatypeProperty rdf:about="http://example.org/onto/prop/google_bigquery_routine_return_table_type">
    <rdfs:label>return_table_type</rdfs:label>
    <rdfs:comment>Optional. Can be set only if routineType = "TABLE_VALUED_FUNCTION".

If absent, the return table type is inferred from definitionBody at query time in each query
that references this routine. If present, then the columns in the evaluated table result will
be cast to match the column types specificed in return table type, at query time.</rdfs:comment>
    <rdfs:domain rdf:resource="http://example.org/onto/class/google_bigquery_routine"/>
    <rdfs:range rdf:resource="http://www.w3.org/2001/XMLSchema#string"/>
  </owl:DatatypeProperty>
  <owl:DatatypeProperty rdf:about="http://example.org/onto/prop/google_bigquery_routine_return_type">
    <rdfs:label>return_type</rdfs:label>
    <rdfs:comment>A JSON schema for the return type. Optional if language = "SQL"; required otherwise.
If absent, the return type is inferred from definitionBody at query time in each query
that references this routine. If present, then the evaluated result will be cast to
the specified returned type at query time. ~>**NOTE**: Because this field expects a JSON
string, any changes to the string will create a diff, even if the JSON itself hasn't
changed. If the API returns a different value for the same schema, e.g. it switche
d the order of values or replaced STRUCT field type with RECORD field type, we currently
cannot suppress the recurring diff this causes. As a workaround, we recommend using
the schema as returned by the API.</rdfs:comment>
    <rdfs:domain rdf:resource="http://example.org/onto/class/google_bigquery_routine"/>
    <rdfs:range rdf:resource="http://www.w3.org/2001/XMLSchema#string"/>
  </owl:DatatypeProperty>
  <owl:DatatypeProperty rdf:about="http://example.org/onto/prop/google_bigquery_routine_routine_id">
    <rdfs:label>routine_id</rdfs:label>
    <rdfs:comment>The ID of the the routine. The ID must contain only letters (a-z, A-Z), numbers (0-9), or underscores (_). The maximum length is 256 characters.</rdfs:comment>
    <rdfs:domain rdf:resource="http://example.org/onto/class/google_bigquery_routine"/>
    <rdfs:range rdf:resource="http://www.w3.org/2001/XMLSchema#string"/>
  </owl:DatatypeProperty>
  <owl:DatatypeProperty rdf:about="http://example.org/onto/prop/google_bigquery_routine_routine_type">
    <rdfs:label>routine_type</rdfs:label>
    <rdfs:comment>The type of routine. Possible values: ["SCALAR_FUNCTION", "PROCEDURE", "TABLE_VALUED_FUNCTION"]</rdfs:comment>
    <rdfs:domain rdf:resource="http://example.org/onto/class/google_bigquery_routine"/>
    <rdfs:range rdf:resource="http://www.w3.org/2001/XMLSchema#string"/>
  </owl:DatatypeProperty>
  <owl:DatatypeProperty rdf:about="http://example.org/onto/prop/google_bigquery_routine_security_mode">
    <rdfs:label>security_mode</rdfs:label>
    <rdfs:comment>Optional. The security mode of the routine, if defined. If not defined, the security mode is automatically determined from the routine's configuration. Possible values: ["DEFINER", "INVOKER"]</rdfs:comment>
    <rdfs:domain rdf:resource="http://example.org/onto/class/google_bigquery_routine"/>
    <rdfs:range rdf:resource="http://www.w3.org/2001/XMLSchema#string"/>
  </owl:DatatypeProperty>
  <owl:DatatypeProperty rdf:about="http://example.org/onto/prop/google_bigquery_routine_argument_kind">
    <rdfs:label>argument_kind</rdfs:label>
    <rdfs:comment>Defaults to FIXED_TYPE. Default value: "FIXED_TYPE" Possible values: ["FIXED_TYPE", "ANY_TYPE"]</rdfs:comment>
    <rdfs:domain rdf:resource="http://example.org/onto/class/google_bigquery_routine"/>
    <rdfs:range rdf:resource="http://www.w3.org/2001/XMLSchema#string"/>
  </owl:DatatypeProperty>
  <owl:DatatypeProperty rdf:about="http://example.org/onto/prop/google_bigquery_routine_data_type">
    <rdfs:label>data_type</rdfs:label>
    <rdfs:comment>A JSON schema for the data type. Required unless argumentKind = ANY_TYPE.
~>**NOTE**: Because this field expects a JSON string, any changes to the string
will create a diff, even if the JSON itself hasn't changed. If the API returns
a different value for the same schema, e.g. it switched the order of values
or replaced STRUCT field type with RECORD field type, we currently cannot
suppress the recurring diff this causes. As a workaround, we recommend using
the schema as returned by the API.</rdfs:comment>
    <rdfs:domain rdf:resource="http://example.org/onto/class/google_bigquery_routine"/>
    <rdfs:range rdf:resource="http://www.w3.org/2001/XMLSchema#string"/>
  </owl:DatatypeProperty>
  <owl:DatatypeProperty rdf:about="http://example.org/onto/prop/google_bigquery_routine_mode">
    <rdfs:label>mode</rdfs:label>
    <rdfs:comment>Specifies whether the argument is input or output. Can be set for procedures only. Possible values: ["IN", "OUT", "INOUT"]</rdfs:comment>
    <rdfs:domain rdf:resource="http://example.org/onto/class/google_bigquery_routine"/>
    <rdfs:range rdf:resource="http://www.w3.org/2001/XMLSchema#string"/>
  </owl:DatatypeProperty>
  <owl:DatatypeProperty rdf:about="http://example.org/onto/prop/google_bigquery_routine_name">
    <rdfs:label>name</rdfs:label>
    <rdfs:comment>The name of this argument. Can be absent for function return argument.</rdfs:comment>
    <rdfs:domain rdf:resource="http://example.org/onto/class/google_bigquery_routine"/>
    <rdfs:range rdf:resource="http://www.w3.org/2001/XMLSchema#string"/>
  </owl:DatatypeProperty>
  <owl:DatatypeProperty rdf:about="http://example.org/onto/prop/google_bigquery_routine_connection">
    <rdfs:label>connection</rdfs:label>
    <rdfs:comment>Fully qualified name of the user-provided connection object which holds
the authentication information to send requests to the remote service.
Format: "projects/{projectId}/locations/{locationId}/connections/{connectionId}"</rdfs:comment>
    <rdfs:domain rdf:resource="http://example.org/onto/class/google_bigquery_routine"/>
    <rdfs:range rdf:resource="http://www.w3.org/2001/XMLSchema#string"/>
  </owl:DatatypeProperty>
  <owl:DatatypeProperty rdf:about="http://example.org/onto/prop/google_bigquery_routine_endpoint">
    <rdfs:label>endpoint</rdfs:label>
    <rdfs:comment>Endpoint of the user-provided remote service, e.g.
'https://us-east1-my_gcf_project.cloudfunctions.net/remote_add'</rdfs:comment>
    <rdfs:domain rdf:resource="http://example.org/onto/class/google_bigquery_routine"/>
    <rdfs:range rdf:resource="http://www.w3.org/2001/XMLSchema#string"/>
  </owl:DatatypeProperty>
  <owl:DatatypeProperty rdf:about="http://example.org/onto/prop/google_bigquery_routine_max_batching_rows">
    <rdfs:label>max_batching_rows</rdfs:label>
    <rdfs:comment>Max number of rows in each batch sent to the remote service. If absent or if 0,
BigQuery dynamically decides the number of rows in a batch.</rdfs:comment>
    <rdfs:domain rdf:resource="http://example.org/onto/class/google_bigquery_routine"/>
    <rdfs:range rdf:resource="http://www.w3.org/2001/XMLSchema#string"/>
  </owl:DatatypeProperty>
  <owl:DatatypeProperty rdf:about="http://example.org/onto/prop/google_bigquery_routine_user_defined_context">
    <rdfs:label>user_defined_context</rdfs:label>
    <rdfs:comment>User-defined context as a set of key/value pairs, which will be sent as function
invocation context together with batched arguments in the requests to the remote
service. The total number of bytes of keys and values must be less than 8KB.

An object containing a list of "key": value pairs. Example:
'{ "name": "wrench", "mass": "1.3kg", "count": "3" }'.</rdfs:comment>
    <rdfs:domain rdf:resource="http://example.org/onto/class/google_bigquery_routine"/>
    <rdfs:range rdf:resource="http://www.w3.org/2001/XMLSchema#string"/>
  </owl:DatatypeProperty>
  <owl:DatatypeProperty rdf:about="http://example.org/onto/prop/google_bigquery_routine_archive_uris">
    <rdfs:label>archive_uris</rdfs:label>
    <rdfs:comment>Archive files to be extracted into the working directory of each executor. For more information about Apache Spark, see Apache Spark.</rdfs:comment>
    <rdfs:domain rdf:resource="http://example.org/onto/class/google_bigquery_routine"/>
    <rdfs:range rdf:resource="http://www.w3.org/2001/XMLSchema#string"/>
  </owl:DatatypeProperty>
  <owl:DatatypeProperty rdf:about="http://example.org/onto/prop/google_bigquery_routine_connection">
    <rdfs:label>connection</rdfs:label>
    <rdfs:comment>Fully qualified name of the user-provided Spark connection object.
Format: "projects/{projectId}/locations/{locationId}/connections/{connectionId}"</rdfs:comment>
    <rdfs:domain rdf:resource="http://example.org/onto/class/google_bigquery_routine"/>
    <rdfs:range rdf:resource="http://www.w3.org/2001/XMLSchema#string"/>
  </owl:DatatypeProperty>
  <owl:DatatypeProperty rdf:about="http://example.org/onto/prop/google_bigquery_routine_container_image">
    <rdfs:label>container_image</rdfs:label>
    <rdfs:comment>Custom container image for the runtime environment.</rdfs:comment>
    <rdfs:domain rdf:resource="http://example.org/onto/class/google_bigquery_routine"/>
    <rdfs:range rdf:resource="http://www.w3.org/2001/XMLSchema#string"/>
  </owl:DatatypeProperty>
  <owl:DatatypeProperty rdf:about="http://example.org/onto/prop/google_bigquery_routine_file_uris">
    <rdfs:label>file_uris</rdfs:label>
    <rdfs:comment>Files to be placed in the working directory of each executor. For more information about Apache Spark, see Apache Spark.</rdfs:comment>
    <rdfs:domain rdf:resource="http://example.org/onto/class/google_bigquery_routine"/>
    <rdfs:range rdf:resource="http://www.w3.org/2001/XMLSchema#string"/>
  </owl:DatatypeProperty>
  <owl:DatatypeProperty rdf:about="http://example.org/onto/prop/google_bigquery_routine_jar_uris">
    <rdfs:label>jar_uris</rdfs:label>
    <rdfs:comment>JARs to include on the driver and executor CLASSPATH. For more information about Apache Spark, see Apache Spark.</rdfs:comment>
    <rdfs:domain rdf:resource="http://example.org/onto/class/google_bigquery_routine"/>
    <rdfs:range rdf:resource="http://www.w3.org/2001/XMLSchema#string"/>
  </owl:DatatypeProperty>
  <owl:DatatypeProperty rdf:about="http://example.org/onto/prop/google_bigquery_routine_main_class">
    <rdfs:label>main_class</rdfs:label>
    <rdfs:comment>The fully qualified name of a class in jarUris, for example, com.example.wordcount.
Exactly one of mainClass and main_jar_uri field should be set for Java/Scala language type.</rdfs:comment>
    <rdfs:domain rdf:resource="http://example.org/onto/class/google_bigquery_routine"/>
    <rdfs:range rdf:resource="http://www.w3.org/2001/XMLSchema#string"/>
  </owl:DatatypeProperty>
  <owl:DatatypeProperty rdf:about="http://example.org/onto/prop/google_bigquery_routine_main_file_uri">
    <rdfs:label>main_file_uri</rdfs:label>
    <rdfs:comment>The main file/jar URI of the Spark application.
Exactly one of the definitionBody field and the mainFileUri field must be set for Python.
Exactly one of mainClass and mainFileUri field should be set for Java/Scala language type.</rdfs:comment>
    <rdfs:domain rdf:resource="http://example.org/onto/class/google_bigquery_routine"/>
    <rdfs:range rdf:resource="http://www.w3.org/2001/XMLSchema#string"/>
  </owl:DatatypeProperty>
  <owl:DatatypeProperty rdf:about="http://example.org/onto/prop/google_bigquery_routine_properties">
    <rdfs:label>properties</rdfs:label>
    <rdfs:comment>Configuration properties as a set of key/value pairs, which will be passed on to the Spark application.
For more information, see Apache Spark and the procedure option list.
An object containing a list of "key": value pairs. Example: { "name": "wrench", "mass": "1.3kg", "count": "3" }.</rdfs:comment>
    <rdfs:domain rdf:resource="http://example.org/onto/class/google_bigquery_routine"/>
    <rdfs:range rdf:resource="http://www.w3.org/2001/XMLSchema#string"/>
  </owl:DatatypeProperty>
  <owl:DatatypeProperty rdf:about="http://example.org/onto/prop/google_bigquery_routine_py_file_uris">
    <rdfs:label>py_file_uris</rdfs:label>
    <rdfs:comment>Python files to be placed on the PYTHONPATH for PySpark application. Supported file types: .py, .egg, and .zip. For more information about Apache Spark, see Apache Spark.</rdfs:comment>
    <rdfs:domain rdf:resource="http://example.org/onto/class/google_bigquery_routine"/>
    <rdfs:range rdf:resource="http://www.w3.org/2001/XMLSchema#string"/>
  </owl:DatatypeProperty>
  <owl:DatatypeProperty rdf:about="http://example.org/onto/prop/google_bigquery_routine_runtime_version">
    <rdfs:label>runtime_version</rdfs:label>
    <rdfs:comment>Runtime version. If not specified, the default runtime version is used.</rdfs:comment>
    <rdfs:domain rdf:resource="http://example.org/onto/class/google_bigquery_routine"/>
    <rdfs:range rdf:resource="http://www.w3.org/2001/XMLSchema#string"/>
  </owl:DatatypeProperty>
  <owl:DatatypeProperty rdf:about="http://example.org/onto/prop/google_bigquery_routine_create">
    <rdfs:label>create</rdfs:label>
    <rdfs:domain rdf:resource="http://example.org/onto/class/google_bigquery_routine"/>
    <rdfs:range rdf:resource="http://www.w3.org/2001/XMLSchema#string"/>
  </owl:DatatypeProperty>
  <owl:DatatypeProperty rdf:about="http://example.org/onto/prop/google_bigquery_routine_delete">
    <rdfs:label>delete</rdfs:label>
    <rdfs:domain rdf:resource="http://example.org/onto/class/google_bigquery_routine"/>
    <rdfs:range rdf:resource="http://www.w3.org/2001/XMLSchema#string"/>
  </owl:DatatypeProperty>
  <owl:DatatypeProperty rdf:about="http://example.org/onto/prop/google_bigquery_routine_update">
    <rdfs:label>update</rdfs:label>
    <rdfs:domain rdf:resource="http://example.org/onto/class/google_bigquery_routine"/>
    <rdfs:range rdf:resource="http://www.w3.org/2001/XMLSchema#string"/>
  </owl:DatatypeProperty>
</rdf:RDF>
