<?xml version="1.0" encoding="UTF-8"?>
<rdf:RDF
  xmlns:rdf="http://www.w3.org/1999/02/22-rdf-syntax-ns#"
  xmlns:rdfs="http://www.w3.org/2000/01/rdf-schema#"
  xmlns:owl="http://www.w3.org/2002/07/owl#"
  xmlns:xsd="http://www.w3.org/2001/XMLSchema#"
  xml:base="http://example.org/onto/">
  <owl:Class rdf:about="http://example.org/onto/class/google_compute_instance_group_manager">
    <rdfs:label>google_compute_instance_group_manager</rdfs:label>
    <rdfs:comment>#
#     ***     AUTO GENERATED CODE    ***    Type: Handwritten     ***
#
# ----------------------------------------------------------------------------
#
#     This code is generated by Magic Modules using the following:
#
#     Source file: https://github.com/GoogleCloudPlatform/magic-modules/tree/main/mmv1/third_party/terraform/website/docs/r/compute_instance_group_manager.html.markdown
#
#     DO NOT EDIT this file directly. Any changes made to this file will be
#     overwritten during the next generation cycle.
#
# ----------------------------------------------------------------------------
subcategory: "Compute Engine"
description: |-
  Manages an Instance Group within GCE.
---</rdfs:comment>
  </owl:Class>
  <owl:DatatypeProperty rdf:about="http://example.org/onto/prop/google_compute_instance_group_manager_base_instance_name">
    <rdfs:label>base_instance_name</rdfs:label>
    <rdfs:comment>The base instance name to use for instances in this group. The value must be a valid RFC1035 name. Supported characters are lowercase letters, numbers, and hyphens (-). Instances are named by appending a hyphen and a random four-character string to the base instance name.</rdfs:comment>
    <rdfs:domain rdf:resource="http://example.org/onto/class/google_compute_instance_group_manager"/>
    <rdfs:range rdf:resource="http://www.w3.org/2001/XMLSchema#string"/>
  </owl:DatatypeProperty>
  <owl:DatatypeProperty rdf:about="http://example.org/onto/prop/google_compute_instance_group_manager_creation_timestamp">
    <rdfs:label>creation_timestamp</rdfs:label>
    <rdfs:comment>Creation timestamp in RFC3339 text format.</rdfs:comment>
    <rdfs:domain rdf:resource="http://example.org/onto/class/google_compute_instance_group_manager"/>
    <rdfs:range rdf:resource="http://www.w3.org/2001/XMLSchema#string"/>
  </owl:DatatypeProperty>
  <owl:DatatypeProperty rdf:about="http://example.org/onto/prop/google_compute_instance_group_manager_description">
    <rdfs:label>description</rdfs:label>
    <rdfs:comment>An optional textual description of the instance group manager.</rdfs:comment>
    <rdfs:domain rdf:resource="http://example.org/onto/class/google_compute_instance_group_manager"/>
    <rdfs:range rdf:resource="http://www.w3.org/2001/XMLSchema#string"/>
  </owl:DatatypeProperty>
  <owl:DatatypeProperty rdf:about="http://example.org/onto/prop/google_compute_instance_group_manager_fingerprint">
    <rdfs:label>fingerprint</rdfs:label>
    <rdfs:comment>The fingerprint of the instance group manager.</rdfs:comment>
    <rdfs:domain rdf:resource="http://example.org/onto/class/google_compute_instance_group_manager"/>
    <rdfs:range rdf:resource="http://www.w3.org/2001/XMLSchema#string"/>
  </owl:DatatypeProperty>
  <owl:DatatypeProperty rdf:about="http://example.org/onto/prop/google_compute_instance_group_manager_id">
    <rdfs:label>id</rdfs:label>
    <rdfs:domain rdf:resource="http://example.org/onto/class/google_compute_instance_group_manager"/>
    <rdfs:range rdf:resource="http://www.w3.org/2001/XMLSchema#string"/>
  </owl:DatatypeProperty>
  <owl:DatatypeProperty rdf:about="http://example.org/onto/prop/google_compute_instance_group_manager_instance_group">
    <rdfs:label>instance_group</rdfs:label>
    <rdfs:comment>The full URL of the instance group created by the manager.</rdfs:comment>
    <rdfs:domain rdf:resource="http://example.org/onto/class/google_compute_instance_group_manager"/>
    <rdfs:range rdf:resource="http://www.w3.org/2001/XMLSchema#string"/>
  </owl:DatatypeProperty>
  <owl:DatatypeProperty rdf:about="http://example.org/onto/prop/google_compute_instance_group_manager_instance_group_manager_id">
    <rdfs:label>instance_group_manager_id</rdfs:label>
    <rdfs:comment>The unique identifier number for the resource. This identifier is defined by the server.</rdfs:comment>
    <rdfs:domain rdf:resource="http://example.org/onto/class/google_compute_instance_group_manager"/>
    <rdfs:range rdf:resource="http://www.w3.org/2001/XMLSchema#string"/>
  </owl:DatatypeProperty>
  <owl:DatatypeProperty rdf:about="http://example.org/onto/prop/google_compute_instance_group_manager_list_managed_instances_results">
    <rdfs:label>list_managed_instances_results</rdfs:label>
    <rdfs:comment>Pagination behavior of the listManagedInstances API method for this managed instance group. Valid values are: "PAGELESS", "PAGINATED". If PAGELESS (default), Pagination is disabled for the group's listManagedInstances API method. maxResults and pageToken query parameters are ignored and all instances are returned in a single response. If PAGINATED, pagination is enabled, maxResults and pageToken query parameters are respected.</rdfs:comment>
    <rdfs:domain rdf:resource="http://example.org/onto/class/google_compute_instance_group_manager"/>
    <rdfs:range rdf:resource="http://www.w3.org/2001/XMLSchema#string"/>
  </owl:DatatypeProperty>
  <owl:DatatypeProperty rdf:about="http://example.org/onto/prop/google_compute_instance_group_manager_name">
    <rdfs:label>name</rdfs:label>
    <rdfs:comment>The name of the instance group manager. Must be 1-63 characters long and comply with RFC1035. Supported characters include lowercase letters, numbers, and hyphens.</rdfs:comment>
    <rdfs:domain rdf:resource="http://example.org/onto/class/google_compute_instance_group_manager"/>
    <rdfs:range rdf:resource="http://www.w3.org/2001/XMLSchema#string"/>
  </owl:DatatypeProperty>
  <owl:DatatypeProperty rdf:about="http://example.org/onto/prop/google_compute_instance_group_manager_operation">
    <rdfs:label>operation</rdfs:label>
    <rdfs:domain rdf:resource="http://example.org/onto/class/google_compute_instance_group_manager"/>
    <rdfs:range rdf:resource="http://www.w3.org/2001/XMLSchema#string"/>
  </owl:DatatypeProperty>
  <owl:DatatypeProperty rdf:about="http://example.org/onto/prop/google_compute_instance_group_manager_project">
    <rdfs:label>project</rdfs:label>
    <rdfs:comment>The ID of the project in which the resource belongs. If it is not provided, the provider project is used.</rdfs:comment>
    <rdfs:domain rdf:resource="http://example.org/onto/class/google_compute_instance_group_manager"/>
    <rdfs:range rdf:resource="http://www.w3.org/2001/XMLSchema#string"/>
  </owl:DatatypeProperty>
  <owl:DatatypeProperty rdf:about="http://example.org/onto/prop/google_compute_instance_group_manager_self_link">
    <rdfs:label>self_link</rdfs:label>
    <rdfs:comment>The URL of the created resource.</rdfs:comment>
    <rdfs:domain rdf:resource="http://example.org/onto/class/google_compute_instance_group_manager"/>
    <rdfs:range rdf:resource="http://www.w3.org/2001/XMLSchema#string"/>
  </owl:DatatypeProperty>
  <owl:DatatypeProperty rdf:about="http://example.org/onto/prop/google_compute_instance_group_manager_status">
    <rdfs:label>status</rdfs:label>
    <rdfs:comment>The status of this managed instance group.</rdfs:comment>
    <rdfs:domain rdf:resource="http://example.org/onto/class/google_compute_instance_group_manager"/>
    <rdfs:range rdf:resource="http://www.w3.org/2001/XMLSchema#string"/>
  </owl:DatatypeProperty>
  <owl:DatatypeProperty rdf:about="http://example.org/onto/prop/google_compute_instance_group_manager_target_pools">
    <rdfs:label>target_pools</rdfs:label>
    <rdfs:comment>The full URL of all target pools to which new instances in the group are added. Updating the target pools attribute does not affect existing instances.</rdfs:comment>
    <rdfs:domain rdf:resource="http://example.org/onto/class/google_compute_instance_group_manager"/>
    <rdfs:range rdf:resource="http://www.w3.org/2001/XMLSchema#string"/>
  </owl:DatatypeProperty>
  <owl:DatatypeProperty rdf:about="http://example.org/onto/prop/google_compute_instance_group_manager_target_size">
    <rdfs:label>target_size</rdfs:label>
    <rdfs:comment>The target number of running instances for this managed instance group. This value should always be explicitly set unless this resource is attached to an autoscaler, in which case it should never be set. Defaults to 0.</rdfs:comment>
    <rdfs:domain rdf:resource="http://example.org/onto/class/google_compute_instance_group_manager"/>
    <rdfs:range rdf:resource="http://www.w3.org/2001/XMLSchema#string"/>
  </owl:DatatypeProperty>
  <owl:DatatypeProperty rdf:about="http://example.org/onto/prop/google_compute_instance_group_manager_target_stopped_size">
    <rdfs:label>target_stopped_size</rdfs:label>
    <rdfs:comment>The target number of stopped instances for this managed instance group.</rdfs:comment>
    <rdfs:domain rdf:resource="http://example.org/onto/class/google_compute_instance_group_manager"/>
    <rdfs:range rdf:resource="http://www.w3.org/2001/XMLSchema#string"/>
  </owl:DatatypeProperty>
  <owl:DatatypeProperty rdf:about="http://example.org/onto/prop/google_compute_instance_group_manager_target_suspended_size">
    <rdfs:label>target_suspended_size</rdfs:label>
    <rdfs:comment>The target number of suspended instances for this managed instance group.</rdfs:comment>
    <rdfs:domain rdf:resource="http://example.org/onto/class/google_compute_instance_group_manager"/>
    <rdfs:range rdf:resource="http://www.w3.org/2001/XMLSchema#string"/>
  </owl:DatatypeProperty>
  <owl:DatatypeProperty rdf:about="http://example.org/onto/prop/google_compute_instance_group_manager_wait_for_instances">
    <rdfs:label>wait_for_instances</rdfs:label>
    <rdfs:comment>Whether to wait for all instances to be created/updated before returning. Note that if this is set to true and the operation does not succeed, Terraform will continue trying until it times out.</rdfs:comment>
    <rdfs:domain rdf:resource="http://example.org/onto/class/google_compute_instance_group_manager"/>
    <rdfs:range rdf:resource="http://www.w3.org/2001/XMLSchema#string"/>
  </owl:DatatypeProperty>
  <owl:DatatypeProperty rdf:about="http://example.org/onto/prop/google_compute_instance_group_manager_wait_for_instances_status">
    <rdfs:label>wait_for_instances_status</rdfs:label>
    <rdfs:comment>When used with wait_for_instances specifies the status to wait for. When STABLE is specified this resource will wait until the instances are stable before returning. When UPDATED is set, it will wait for the version target to be reached and any per instance configs to be effective and all instances configs to be effective as well as all instances to be stable before returning.</rdfs:comment>
    <rdfs:domain rdf:resource="http://example.org/onto/class/google_compute_instance_group_manager"/>
    <rdfs:range rdf:resource="http://www.w3.org/2001/XMLSchema#string"/>
  </owl:DatatypeProperty>
  <owl:DatatypeProperty rdf:about="http://example.org/onto/prop/google_compute_instance_group_manager_zone">
    <rdfs:label>zone</rdfs:label>
    <rdfs:comment>The zone that instances in this group should be created in.</rdfs:comment>
    <rdfs:domain rdf:resource="http://example.org/onto/class/google_compute_instance_group_manager"/>
    <rdfs:range rdf:resource="http://www.w3.org/2001/XMLSchema#string"/>
  </owl:DatatypeProperty>
  <owl:DatatypeProperty rdf:about="http://example.org/onto/prop/google_compute_instance_group_manager_labels">
    <rdfs:label>labels</rdfs:label>
    <rdfs:comment>The label key-value pairs that you want to patch onto the instance,</rdfs:comment>
    <rdfs:domain rdf:resource="http://example.org/onto/class/google_compute_instance_group_manager"/>
    <rdfs:range rdf:resource="http://www.w3.org/2001/XMLSchema#string"/>
  </owl:DatatypeProperty>
  <owl:DatatypeProperty rdf:about="http://example.org/onto/prop/google_compute_instance_group_manager_metadata">
    <rdfs:label>metadata</rdfs:label>
    <rdfs:comment>The metadata key-value pairs that you want to patch onto the instance. For more information, see Project and instance metadata,</rdfs:comment>
    <rdfs:domain rdf:resource="http://example.org/onto/class/google_compute_instance_group_manager"/>
    <rdfs:range rdf:resource="http://www.w3.org/2001/XMLSchema#string"/>
  </owl:DatatypeProperty>
  <owl:DatatypeProperty rdf:about="http://example.org/onto/prop/google_compute_instance_group_manager_health_check">
    <rdfs:label>health_check</rdfs:label>
    <rdfs:comment>The health check resource that signals autohealing.</rdfs:comment>
    <rdfs:domain rdf:resource="http://example.org/onto/class/google_compute_instance_group_manager"/>
    <rdfs:range rdf:resource="http://www.w3.org/2001/XMLSchema#string"/>
  </owl:DatatypeProperty>
  <owl:DatatypeProperty rdf:about="http://example.org/onto/prop/google_compute_instance_group_manager_initial_delay_sec">
    <rdfs:label>initial_delay_sec</rdfs:label>
    <rdfs:comment>The number of seconds that the managed instance group waits before it applies autohealing policies to new instances or recently recreated instances. Between 0 and 3600.</rdfs:comment>
    <rdfs:domain rdf:resource="http://example.org/onto/class/google_compute_instance_group_manager"/>
    <rdfs:range rdf:resource="http://www.w3.org/2001/XMLSchema#string"/>
  </owl:DatatypeProperty>
  <owl:DatatypeProperty rdf:about="http://example.org/onto/prop/google_compute_instance_group_manager_default_action_on_failure">
    <rdfs:label>default_action_on_failure</rdfs:label>
    <rdfs:comment>Default behavior for all instance or health check failures.</rdfs:comment>
    <rdfs:domain rdf:resource="http://example.org/onto/class/google_compute_instance_group_manager"/>
    <rdfs:range rdf:resource="http://www.w3.org/2001/XMLSchema#string"/>
  </owl:DatatypeProperty>
  <owl:DatatypeProperty rdf:about="http://example.org/onto/prop/google_compute_instance_group_manager_force_update_on_repair">
    <rdfs:label>force_update_on_repair</rdfs:label>
    <rdfs:comment>Specifies whether to apply the group's latest configuration when repairing a VM. Valid options are: YES, NO. If YES and you updated the group's instance template or per-instance configurations after the VM was created, then these changes are applied when VM is repaired. If NO (default), then updates are applied in accordance with the group's update policy type.</rdfs:comment>
    <rdfs:domain rdf:resource="http://example.org/onto/class/google_compute_instance_group_manager"/>
    <rdfs:range rdf:resource="http://www.w3.org/2001/XMLSchema#string"/>
  </owl:DatatypeProperty>
  <owl:DatatypeProperty rdf:about="http://example.org/onto/prop/google_compute_instance_group_manager_name">
    <rdfs:label>name</rdfs:label>
    <rdfs:comment>The name of the port.</rdfs:comment>
    <rdfs:domain rdf:resource="http://example.org/onto/class/google_compute_instance_group_manager"/>
    <rdfs:range rdf:resource="http://www.w3.org/2001/XMLSchema#string"/>
  </owl:DatatypeProperty>
  <owl:DatatypeProperty rdf:about="http://example.org/onto/prop/google_compute_instance_group_manager_port">
    <rdfs:label>port</rdfs:label>
    <rdfs:comment>The port number.</rdfs:comment>
    <rdfs:domain rdf:resource="http://example.org/onto/class/google_compute_instance_group_manager"/>
    <rdfs:range rdf:resource="http://www.w3.org/2001/XMLSchema#string"/>
  </owl:DatatypeProperty>
  <owl:DatatypeProperty rdf:about="http://example.org/onto/prop/google_compute_instance_group_manager_workload_policy">
    <rdfs:label>workload_policy</rdfs:label>
    <rdfs:comment>The URL of the workload policy that is specified for this managed instance group. It can be a full or partial URL.</rdfs:comment>
    <rdfs:domain rdf:resource="http://example.org/onto/class/google_compute_instance_group_manager"/>
    <rdfs:range rdf:resource="http://www.w3.org/2001/XMLSchema#string"/>
  </owl:DatatypeProperty>
  <owl:DatatypeProperty rdf:about="http://example.org/onto/prop/google_compute_instance_group_manager_initial_delay_sec">
    <rdfs:label>initial_delay_sec</rdfs:label>
    <rdfs:comment>Specifies the number of seconds that the MIG should wait to suspend or stop a VM after that VM was created. The initial delay gives the initialization script the time to prepare your VM for a quick scale out. The value of initial delay must be between 0 and 3600 seconds. The default value is 0.</rdfs:comment>
    <rdfs:domain rdf:resource="http://example.org/onto/class/google_compute_instance_group_manager"/>
    <rdfs:range rdf:resource="http://www.w3.org/2001/XMLSchema#string"/>
  </owl:DatatypeProperty>
  <owl:DatatypeProperty rdf:about="http://example.org/onto/prop/google_compute_instance_group_manager_mode">
    <rdfs:label>mode</rdfs:label>
    <rdfs:comment>Defines how a MIG resumes or starts VMs from a standby pool when the group scales out. The default mode is "MANUAL".</rdfs:comment>
    <rdfs:domain rdf:resource="http://example.org/onto/class/google_compute_instance_group_manager"/>
    <rdfs:range rdf:resource="http://www.w3.org/2001/XMLSchema#string"/>
  </owl:DatatypeProperty>
  <owl:DatatypeProperty rdf:about="http://example.org/onto/prop/google_compute_instance_group_manager_delete_rule">
    <rdfs:label>delete_rule</rdfs:label>
    <rdfs:comment>A value that prescribes what should happen to the stateful disk when the VM instance is deleted. The available options are NEVER and ON_PERMANENT_INSTANCE_DELETION. NEVER - detach the disk when the VM is deleted, but do not delete the disk. ON_PERMANENT_INSTANCE_DELETION will delete the stateful disk when the VM is permanently deleted from the instance group. The default is NEVER.</rdfs:comment>
    <rdfs:domain rdf:resource="http://example.org/onto/class/google_compute_instance_group_manager"/>
    <rdfs:range rdf:resource="http://www.w3.org/2001/XMLSchema#string"/>
  </owl:DatatypeProperty>
  <owl:DatatypeProperty rdf:about="http://example.org/onto/prop/google_compute_instance_group_manager_device_name">
    <rdfs:label>device_name</rdfs:label>
    <rdfs:comment>The device name of the disk to be attached.</rdfs:comment>
    <rdfs:domain rdf:resource="http://example.org/onto/class/google_compute_instance_group_manager"/>
    <rdfs:range rdf:resource="http://www.w3.org/2001/XMLSchema#string"/>
  </owl:DatatypeProperty>
  <owl:DatatypeProperty rdf:about="http://example.org/onto/prop/google_compute_instance_group_manager_delete_rule">
    <rdfs:label>delete_rule</rdfs:label>
    <rdfs:comment>A value that prescribes what should happen to an associated static Address resource when a VM instance is permanently deleted. The available options are NEVER and ON_PERMANENT_INSTANCE_DELETION. NEVER - detach the IP when the VM is deleted, but do not delete the address resource. ON_PERMANENT_INSTANCE_DELETION will delete the stateful address when the VM is permanently deleted from the instance group. The default is NEVER.</rdfs:comment>
    <rdfs:domain rdf:resource="http://example.org/onto/class/google_compute_instance_group_manager"/>
    <rdfs:range rdf:resource="http://www.w3.org/2001/XMLSchema#string"/>
  </owl:DatatypeProperty>
  <owl:DatatypeProperty rdf:about="http://example.org/onto/prop/google_compute_instance_group_manager_interface_name">
    <rdfs:label>interface_name</rdfs:label>
    <rdfs:comment>The network interface name</rdfs:comment>
    <rdfs:domain rdf:resource="http://example.org/onto/class/google_compute_instance_group_manager"/>
    <rdfs:range rdf:resource="http://www.w3.org/2001/XMLSchema#string"/>
  </owl:DatatypeProperty>
  <owl:DatatypeProperty rdf:about="http://example.org/onto/prop/google_compute_instance_group_manager_delete_rule">
    <rdfs:label>delete_rule</rdfs:label>
    <rdfs:comment>A value that prescribes what should happen to an associated static Address resource when a VM instance is permanently deleted. The available options are NEVER and ON_PERMANENT_INSTANCE_DELETION. NEVER - detach the IP when the VM is deleted, but do not delete the address resource. ON_PERMANENT_INSTANCE_DELETION will delete the stateful address when the VM is permanently deleted from the instance group. The default is NEVER.</rdfs:comment>
    <rdfs:domain rdf:resource="http://example.org/onto/class/google_compute_instance_group_manager"/>
    <rdfs:range rdf:resource="http://www.w3.org/2001/XMLSchema#string"/>
  </owl:DatatypeProperty>
  <owl:DatatypeProperty rdf:about="http://example.org/onto/prop/google_compute_instance_group_manager_interface_name">
    <rdfs:label>interface_name</rdfs:label>
    <rdfs:comment>The network interface name</rdfs:comment>
    <rdfs:domain rdf:resource="http://example.org/onto/class/google_compute_instance_group_manager"/>
    <rdfs:range rdf:resource="http://www.w3.org/2001/XMLSchema#string"/>
  </owl:DatatypeProperty>
  <owl:DatatypeProperty rdf:about="http://example.org/onto/prop/google_compute_instance_group_manager_create">
    <rdfs:label>create</rdfs:label>
    <rdfs:domain rdf:resource="http://example.org/onto/class/google_compute_instance_group_manager"/>
    <rdfs:range rdf:resource="http://www.w3.org/2001/XMLSchema#string"/>
  </owl:DatatypeProperty>
  <owl:DatatypeProperty rdf:about="http://example.org/onto/prop/google_compute_instance_group_manager_delete">
    <rdfs:label>delete</rdfs:label>
    <rdfs:domain rdf:resource="http://example.org/onto/class/google_compute_instance_group_manager"/>
    <rdfs:range rdf:resource="http://www.w3.org/2001/XMLSchema#string"/>
  </owl:DatatypeProperty>
  <owl:DatatypeProperty rdf:about="http://example.org/onto/prop/google_compute_instance_group_manager_update">
    <rdfs:label>update</rdfs:label>
    <rdfs:domain rdf:resource="http://example.org/onto/class/google_compute_instance_group_manager"/>
    <rdfs:range rdf:resource="http://www.w3.org/2001/XMLSchema#string"/>
  </owl:DatatypeProperty>
  <owl:DatatypeProperty rdf:about="http://example.org/onto/prop/google_compute_instance_group_manager_max_surge_fixed">
    <rdfs:label>max_surge_fixed</rdfs:label>
    <rdfs:comment>Specifies a fixed number of VM instances. This must be a positive integer. Conflicts with max_surge_percent. Both cannot be 0</rdfs:comment>
    <rdfs:domain rdf:resource="http://example.org/onto/class/google_compute_instance_group_manager"/>
    <rdfs:range rdf:resource="http://www.w3.org/2001/XMLSchema#string"/>
  </owl:DatatypeProperty>
  <owl:DatatypeProperty rdf:about="http://example.org/onto/prop/google_compute_instance_group_manager_max_surge_percent">
    <rdfs:label>max_surge_percent</rdfs:label>
    <rdfs:comment>Specifies a percentage of instances between 0 to 100%, inclusive. For example, specify 80 for 80%. Conflicts with max_surge_fixed.</rdfs:comment>
    <rdfs:domain rdf:resource="http://example.org/onto/class/google_compute_instance_group_manager"/>
    <rdfs:range rdf:resource="http://www.w3.org/2001/XMLSchema#string"/>
  </owl:DatatypeProperty>
  <owl:DatatypeProperty rdf:about="http://example.org/onto/prop/google_compute_instance_group_manager_max_unavailable_fixed">
    <rdfs:label>max_unavailable_fixed</rdfs:label>
    <rdfs:comment>Specifies a fixed number of VM instances. This must be a positive integer.</rdfs:comment>
    <rdfs:domain rdf:resource="http://example.org/onto/class/google_compute_instance_group_manager"/>
    <rdfs:range rdf:resource="http://www.w3.org/2001/XMLSchema#string"/>
  </owl:DatatypeProperty>
  <owl:DatatypeProperty rdf:about="http://example.org/onto/prop/google_compute_instance_group_manager_max_unavailable_percent">
    <rdfs:label>max_unavailable_percent</rdfs:label>
    <rdfs:comment>Specifies a percentage of instances between 0 to 100%, inclusive. For example, specify 80 for 80%.</rdfs:comment>
    <rdfs:domain rdf:resource="http://example.org/onto/class/google_compute_instance_group_manager"/>
    <rdfs:range rdf:resource="http://www.w3.org/2001/XMLSchema#string"/>
  </owl:DatatypeProperty>
  <owl:DatatypeProperty rdf:about="http://example.org/onto/prop/google_compute_instance_group_manager_minimal_action">
    <rdfs:label>minimal_action</rdfs:label>
    <rdfs:comment>Minimal action to be taken on an instance. You can specify either NONE to forbid any actions, REFRESH to update without stopping instances, RESTART to restart existing instances or REPLACE to delete and create new instances from the target template. If you specify a REFRESH, the Updater will attempt to perform that action only. However, if the Updater determines that the minimal action you specify is not enough to perform the update, it might perform a more disruptive action.</rdfs:comment>
    <rdfs:domain rdf:resource="http://example.org/onto/class/google_compute_instance_group_manager"/>
    <rdfs:range rdf:resource="http://www.w3.org/2001/XMLSchema#string"/>
  </owl:DatatypeProperty>
  <owl:DatatypeProperty rdf:about="http://example.org/onto/prop/google_compute_instance_group_manager_most_disruptive_allowed_action">
    <rdfs:label>most_disruptive_allowed_action</rdfs:label>
    <rdfs:comment>Most disruptive action that is allowed to be taken on an instance. You can specify either NONE to forbid any actions, REFRESH to allow actions that do not need instance restart, RESTART to allow actions that can be applied without instance replacing or REPLACE to allow all possible actions. If the Updater determines that the minimal update action needed is more disruptive than most disruptive allowed action you specify it will not perform the update at all.</rdfs:comment>
    <rdfs:domain rdf:resource="http://example.org/onto/class/google_compute_instance_group_manager"/>
    <rdfs:range rdf:resource="http://www.w3.org/2001/XMLSchema#string"/>
  </owl:DatatypeProperty>
  <owl:DatatypeProperty rdf:about="http://example.org/onto/prop/google_compute_instance_group_manager_replacement_method">
    <rdfs:label>replacement_method</rdfs:label>
    <rdfs:comment>The instance replacement method for managed instance groups. Valid values are: "RECREATE", "SUBSTITUTE". If SUBSTITUTE (default), the group replaces VM instances with new instances that have randomly generated names. If RECREATE, instance names are preserved.  You must also set max_unavailable_fixed or max_unavailable_percent to be greater than 0.</rdfs:comment>
    <rdfs:domain rdf:resource="http://example.org/onto/class/google_compute_instance_group_manager"/>
    <rdfs:range rdf:resource="http://www.w3.org/2001/XMLSchema#string"/>
  </owl:DatatypeProperty>
  <owl:DatatypeProperty rdf:about="http://example.org/onto/prop/google_compute_instance_group_manager_type">
    <rdfs:label>type</rdfs:label>
    <rdfs:comment>The type of update process. You can specify either PROACTIVE so that the instance group manager proactively executes actions in order to bring instances to their target versions or OPPORTUNISTIC so that no action is proactively executed but the update will be performed as part of other actions (for example, resizes or recreateInstances calls).</rdfs:comment>
    <rdfs:domain rdf:resource="http://example.org/onto/class/google_compute_instance_group_manager"/>
    <rdfs:range rdf:resource="http://www.w3.org/2001/XMLSchema#string"/>
  </owl:DatatypeProperty>
  <owl:DatatypeProperty rdf:about="http://example.org/onto/prop/google_compute_instance_group_manager_instance_template">
    <rdfs:label>instance_template</rdfs:label>
    <rdfs:comment>The full URL to an instance template from which all new instances of this version will be created.</rdfs:comment>
    <rdfs:domain rdf:resource="http://example.org/onto/class/google_compute_instance_group_manager"/>
    <rdfs:range rdf:resource="http://www.w3.org/2001/XMLSchema#string"/>
  </owl:DatatypeProperty>
  <owl:DatatypeProperty rdf:about="http://example.org/onto/prop/google_compute_instance_group_manager_name">
    <rdfs:label>name</rdfs:label>
    <rdfs:comment>Version name.</rdfs:comment>
    <rdfs:domain rdf:resource="http://example.org/onto/class/google_compute_instance_group_manager"/>
    <rdfs:range rdf:resource="http://www.w3.org/2001/XMLSchema#string"/>
  </owl:DatatypeProperty>
  <owl:DatatypeProperty rdf:about="http://example.org/onto/prop/google_compute_instance_group_manager_fixed">
    <rdfs:label>fixed</rdfs:label>
    <rdfs:comment>The number of instances which are managed for this version. Conflicts with percent.</rdfs:comment>
    <rdfs:domain rdf:resource="http://example.org/onto/class/google_compute_instance_group_manager"/>
    <rdfs:range rdf:resource="http://www.w3.org/2001/XMLSchema#string"/>
  </owl:DatatypeProperty>
  <owl:DatatypeProperty rdf:about="http://example.org/onto/prop/google_compute_instance_group_manager_percent">
    <rdfs:label>percent</rdfs:label>
    <rdfs:comment>The number of instances (calculated as percentage) which are managed for this version. Conflicts with fixed. Note that when using percent, rounding will be in favor of explicitly set target_size values; a managed instance group with 2 instances and 2 versions, one of which has a target_size.percent of 60 will create 2 instances of that version.</rdfs:comment>
    <rdfs:domain rdf:resource="http://example.org/onto/class/google_compute_instance_group_manager"/>
    <rdfs:range rdf:resource="http://www.w3.org/2001/XMLSchema#string"/>
  </owl:DatatypeProperty>
</rdf:RDF>
