<?xml version="1.0" encoding="UTF-8"?>
<rdf:RDF
  xmlns:rdf="http://www.w3.org/1999/02/22-rdf-syntax-ns#"
  xmlns:rdfs="http://www.w3.org/2000/01/rdf-schema#"
  xmlns:owl="http://www.w3.org/2002/07/owl#"
  xmlns:xsd="http://www.w3.org/2001/XMLSchema#"
  xml:base="http://example.org/onto/">
  <owl:Class rdf:about="http://example.org/onto/class/google_iam_workforce_pool_provider_scim_tenant">
    <rdfs:label>google_iam_workforce_pool_provider_scim_tenant</rdfs:label>
    <rdfs:comment>#
#     ***     AUTO GENERATED CODE    ***    Type: MMv1     ***
#
# ----------------------------------------------------------------------------
#
#     This code is generated by Magic Modules using the following:
#
#     Configuration: https:#github.com/GoogleCloudPlatform/magic-modules/tree/main/mmv1/products/iamworkforcepool/WorkforcePoolProviderScimTenant.yaml
#     Template:      https:#github.com/GoogleCloudPlatform/magic-modules/tree/main/mmv1/templates/terraform/resource.html.markdown.tmpl
#
#     DO NOT EDIT this file directly. Any changes made to this file will be
#     overwritten during the next generation cycle.
#
# ----------------------------------------------------------------------------
subcategory: "Cloud IAM"
description: |-
  Represents a SCIM tenant configuration for a Workforce Pool Provider.
---</rdfs:comment>
  </owl:Class>
  <owl:DatatypeProperty rdf:about="http://example.org/onto/prop/google_iam_workforce_pool_provider_scim_tenant_base_uri">
    <rdfs:label>base_uri</rdfs:label>
    <rdfs:comment>Represents the base URI as defined in [RFC 7644, Section
1.3](https://datatracker.ietf.org/doc/html/rfc7644#section-1.3). Clients
must use this as the root address for managing resources under the tenant.
Format:
https://iamscim.googleapis.com/{version}/{tenant_id}/</rdfs:comment>
    <rdfs:domain rdf:resource="http://example.org/onto/class/google_iam_workforce_pool_provider_scim_tenant"/>
    <rdfs:range rdf:resource="http://www.w3.org/2001/XMLSchema#string"/>
  </owl:DatatypeProperty>
  <owl:DatatypeProperty rdf:about="http://example.org/onto/prop/google_iam_workforce_pool_provider_scim_tenant_description">
    <rdfs:label>description</rdfs:label>
    <rdfs:comment>A user-specified description of the provider. Cannot exceed 256 characters.</rdfs:comment>
    <rdfs:domain rdf:resource="http://example.org/onto/class/google_iam_workforce_pool_provider_scim_tenant"/>
    <rdfs:range rdf:resource="http://www.w3.org/2001/XMLSchema#string"/>
  </owl:DatatypeProperty>
  <owl:DatatypeProperty rdf:about="http://example.org/onto/prop/google_iam_workforce_pool_provider_scim_tenant_display_name">
    <rdfs:label>display_name</rdfs:label>
    <rdfs:comment>A user-specified display name for the scim tenant. Cannot exceed 32 characters.</rdfs:comment>
    <rdfs:domain rdf:resource="http://example.org/onto/class/google_iam_workforce_pool_provider_scim_tenant"/>
    <rdfs:range rdf:resource="http://www.w3.org/2001/XMLSchema#string"/>
  </owl:DatatypeProperty>
  <owl:DatatypeProperty rdf:about="http://example.org/onto/prop/google_iam_workforce_pool_provider_scim_tenant_id">
    <rdfs:label>id</rdfs:label>
    <rdfs:domain rdf:resource="http://example.org/onto/class/google_iam_workforce_pool_provider_scim_tenant"/>
    <rdfs:range rdf:resource="http://www.w3.org/2001/XMLSchema#string"/>
  </owl:DatatypeProperty>
  <owl:DatatypeProperty rdf:about="http://example.org/onto/prop/google_iam_workforce_pool_provider_scim_tenant_location">
    <rdfs:label>location</rdfs:label>
    <rdfs:comment>The location for the resource.</rdfs:comment>
    <rdfs:domain rdf:resource="http://example.org/onto/class/google_iam_workforce_pool_provider_scim_tenant"/>
    <rdfs:range rdf:resource="http://www.w3.org/2001/XMLSchema#string"/>
  </owl:DatatypeProperty>
  <owl:DatatypeProperty rdf:about="http://example.org/onto/prop/google_iam_workforce_pool_provider_scim_tenant_name">
    <rdfs:label>name</rdfs:label>
    <rdfs:comment>Identifier. The resource name of the scim tenant.
Format: 'locations/{location}/workforcePools/{workforce_pool}/providers/{workforce_pool_provider}/scimTenants/{scim_tenant_id}</rdfs:comment>
    <rdfs:domain rdf:resource="http://example.org/onto/class/google_iam_workforce_pool_provider_scim_tenant"/>
    <rdfs:range rdf:resource="http://www.w3.org/2001/XMLSchema#string"/>
  </owl:DatatypeProperty>
  <owl:DatatypeProperty rdf:about="http://example.org/onto/prop/google_iam_workforce_pool_provider_scim_tenant_provider_id">
    <rdfs:label>provider_id</rdfs:label>
    <rdfs:comment>The ID of the provider.</rdfs:comment>
    <rdfs:domain rdf:resource="http://example.org/onto/class/google_iam_workforce_pool_provider_scim_tenant"/>
    <rdfs:range rdf:resource="http://www.w3.org/2001/XMLSchema#string"/>
  </owl:DatatypeProperty>
  <owl:DatatypeProperty rdf:about="http://example.org/onto/prop/google_iam_workforce_pool_provider_scim_tenant_scim_tenant_id">
    <rdfs:label>scim_tenant_id</rdfs:label>
    <rdfs:comment>The ID to use for the SCIM tenant, which becomes the final component of the resource name. This value must be 4-32 characters, and may contain the characters [a-z0-9-].</rdfs:comment>
    <rdfs:domain rdf:resource="http://example.org/onto/class/google_iam_workforce_pool_provider_scim_tenant"/>
    <rdfs:range rdf:resource="http://www.w3.org/2001/XMLSchema#string"/>
  </owl:DatatypeProperty>
  <owl:DatatypeProperty rdf:about="http://example.org/onto/prop/google_iam_workforce_pool_provider_scim_tenant_state">
    <rdfs:label>state</rdfs:label>
    <rdfs:comment>The current state of the scim tenant.
* STATE_UNSPECIFIED: State unspecified.
* ACTIVE: The scim tenant is active and may be used to validate authentication credentials.
* DELETED: The scim tenant is soft-deleted. Soft-deleted scim tenants are permanently
  deleted after approximately 30 days.</rdfs:comment>
    <rdfs:domain rdf:resource="http://example.org/onto/class/google_iam_workforce_pool_provider_scim_tenant"/>
    <rdfs:range rdf:resource="http://www.w3.org/2001/XMLSchema#string"/>
  </owl:DatatypeProperty>
  <owl:DatatypeProperty rdf:about="http://example.org/onto/prop/google_iam_workforce_pool_provider_scim_tenant_workforce_pool_id">
    <rdfs:label>workforce_pool_id</rdfs:label>
    <rdfs:comment>The ID of the workforce pool.</rdfs:comment>
    <rdfs:domain rdf:resource="http://example.org/onto/class/google_iam_workforce_pool_provider_scim_tenant"/>
    <rdfs:range rdf:resource="http://www.w3.org/2001/XMLSchema#string"/>
  </owl:DatatypeProperty>
  <owl:DatatypeProperty rdf:about="http://example.org/onto/prop/google_iam_workforce_pool_provider_scim_tenant_create">
    <rdfs:label>create</rdfs:label>
    <rdfs:domain rdf:resource="http://example.org/onto/class/google_iam_workforce_pool_provider_scim_tenant"/>
    <rdfs:range rdf:resource="http://www.w3.org/2001/XMLSchema#string"/>
  </owl:DatatypeProperty>
  <owl:DatatypeProperty rdf:about="http://example.org/onto/prop/google_iam_workforce_pool_provider_scim_tenant_delete">
    <rdfs:label>delete</rdfs:label>
    <rdfs:domain rdf:resource="http://example.org/onto/class/google_iam_workforce_pool_provider_scim_tenant"/>
    <rdfs:range rdf:resource="http://www.w3.org/2001/XMLSchema#string"/>
  </owl:DatatypeProperty>
  <owl:DatatypeProperty rdf:about="http://example.org/onto/prop/google_iam_workforce_pool_provider_scim_tenant_update">
    <rdfs:label>update</rdfs:label>
    <rdfs:domain rdf:resource="http://example.org/onto/class/google_iam_workforce_pool_provider_scim_tenant"/>
    <rdfs:range rdf:resource="http://www.w3.org/2001/XMLSchema#string"/>
  </owl:DatatypeProperty>
</rdf:RDF>
