<?xml version="1.0" encoding="UTF-8"?>
<rdf:RDF
  xmlns:rdf="http://www.w3.org/1999/02/22-rdf-syntax-ns#"
  xmlns:rdfs="http://www.w3.org/2000/01/rdf-schema#"
  xmlns:owl="http://www.w3.org/2002/07/owl#"
  xmlns:xsd="http://www.w3.org/2001/XMLSchema#"
  xml:base="http://example.org/onto/">
  <owl:Class rdf:about="http://example.org/onto/class/google_os_config_patch_deployment">
    <rdfs:label>google_os_config_patch_deployment</rdfs:label>
    <rdfs:comment>#
#     ***     AUTO GENERATED CODE    ***    Type: MMv1     ***
#
# ----------------------------------------------------------------------------
#
#     This code is generated by Magic Modules using the following:
#
#     Configuration: https:#github.com/GoogleCloudPlatform/magic-modules/tree/main/mmv1/products/osconfig/PatchDeployment.yaml
#     Template:      https:#github.com/GoogleCloudPlatform/magic-modules/tree/main/mmv1/templates/terraform/resource.html.markdown.tmpl
#
#     DO NOT EDIT this file directly. Any changes made to this file will be
#     overwritten during the next generation cycle.
#
# ----------------------------------------------------------------------------
subcategory: "OS Config"
description: |-
  Patch deployments are configurations that individual patch jobs use to complete a patch.
---</rdfs:comment>
  </owl:Class>
  <owl:DatatypeProperty rdf:about="http://example.org/onto/prop/google_os_config_patch_deployment_create_time">
    <rdfs:label>create_time</rdfs:label>
    <rdfs:comment>Time the patch deployment was created. Timestamp is in RFC3339 text format.
A timestamp in RFC3339 UTC "Zulu" format, accurate to nanoseconds. Example: "2014-10-02T15:01:23.045123456Z".</rdfs:comment>
    <rdfs:domain rdf:resource="http://example.org/onto/class/google_os_config_patch_deployment"/>
    <rdfs:range rdf:resource="http://www.w3.org/2001/XMLSchema#string"/>
  </owl:DatatypeProperty>
  <owl:DatatypeProperty rdf:about="http://example.org/onto/prop/google_os_config_patch_deployment_description">
    <rdfs:label>description</rdfs:label>
    <rdfs:comment>Description of the patch deployment. Length of the description is limited to 1024 characters.</rdfs:comment>
    <rdfs:domain rdf:resource="http://example.org/onto/class/google_os_config_patch_deployment"/>
    <rdfs:range rdf:resource="http://www.w3.org/2001/XMLSchema#string"/>
  </owl:DatatypeProperty>
  <owl:DatatypeProperty rdf:about="http://example.org/onto/prop/google_os_config_patch_deployment_duration">
    <rdfs:label>duration</rdfs:label>
    <rdfs:comment>Duration of the patch. After the duration ends, the patch times out.
A duration in seconds with up to nine fractional digits, terminated by 's'. Example: "3.5s"</rdfs:comment>
    <rdfs:domain rdf:resource="http://example.org/onto/class/google_os_config_patch_deployment"/>
    <rdfs:range rdf:resource="http://www.w3.org/2001/XMLSchema#string"/>
  </owl:DatatypeProperty>
  <owl:DatatypeProperty rdf:about="http://example.org/onto/prop/google_os_config_patch_deployment_id">
    <rdfs:label>id</rdfs:label>
    <rdfs:domain rdf:resource="http://example.org/onto/class/google_os_config_patch_deployment"/>
    <rdfs:range rdf:resource="http://www.w3.org/2001/XMLSchema#string"/>
  </owl:DatatypeProperty>
  <owl:DatatypeProperty rdf:about="http://example.org/onto/prop/google_os_config_patch_deployment_last_execute_time">
    <rdfs:label>last_execute_time</rdfs:label>
    <rdfs:comment>The last time a patch job was started by this deployment. Timestamp is in RFC3339 text format.
A timestamp in RFC3339 UTC "Zulu" format, accurate to nanoseconds. Example: "2014-10-02T15:01:23.045123456Z".</rdfs:comment>
    <rdfs:domain rdf:resource="http://example.org/onto/class/google_os_config_patch_deployment"/>
    <rdfs:range rdf:resource="http://www.w3.org/2001/XMLSchema#string"/>
  </owl:DatatypeProperty>
  <owl:DatatypeProperty rdf:about="http://example.org/onto/prop/google_os_config_patch_deployment_name">
    <rdfs:label>name</rdfs:label>
    <rdfs:comment>Unique name for the patch deployment resource in a project.
The patch deployment name is in the form: projects/{project_id}/patchDeployments/{patchDeploymentId}.</rdfs:comment>
    <rdfs:domain rdf:resource="http://example.org/onto/class/google_os_config_patch_deployment"/>
    <rdfs:range rdf:resource="http://www.w3.org/2001/XMLSchema#string"/>
  </owl:DatatypeProperty>
  <owl:DatatypeProperty rdf:about="http://example.org/onto/prop/google_os_config_patch_deployment_patch_deployment_id">
    <rdfs:label>patch_deployment_id</rdfs:label>
    <rdfs:comment>A name for the patch deployment in the project. When creating a name the following rules apply:
* Must contain only lowercase letters, numbers, and hyphens.
* Must start with a letter.
* Must be between 1-63 characters.
* Must end with a number or a letter.
* Must be unique within the project.</rdfs:comment>
    <rdfs:domain rdf:resource="http://example.org/onto/class/google_os_config_patch_deployment"/>
    <rdfs:range rdf:resource="http://www.w3.org/2001/XMLSchema#string"/>
  </owl:DatatypeProperty>
  <owl:DatatypeProperty rdf:about="http://example.org/onto/prop/google_os_config_patch_deployment_project">
    <rdfs:label>project</rdfs:label>
    <rdfs:domain rdf:resource="http://example.org/onto/class/google_os_config_patch_deployment"/>
    <rdfs:range rdf:resource="http://www.w3.org/2001/XMLSchema#string"/>
  </owl:DatatypeProperty>
  <owl:DatatypeProperty rdf:about="http://example.org/onto/prop/google_os_config_patch_deployment_update_time">
    <rdfs:label>update_time</rdfs:label>
    <rdfs:comment>Time the patch deployment was last updated. Timestamp is in RFC3339 text format.
A timestamp in RFC3339 UTC "Zulu" format, accurate to nanoseconds. Example: "2014-10-02T15:01:23.045123456Z".</rdfs:comment>
    <rdfs:domain rdf:resource="http://example.org/onto/class/google_os_config_patch_deployment"/>
    <rdfs:range rdf:resource="http://www.w3.org/2001/XMLSchema#string"/>
  </owl:DatatypeProperty>
  <owl:DatatypeProperty rdf:about="http://example.org/onto/prop/google_os_config_patch_deployment_all">
    <rdfs:label>all</rdfs:label>
    <rdfs:comment>Target all VM instances in the project. If true, no other criteria is permitted.</rdfs:comment>
    <rdfs:domain rdf:resource="http://example.org/onto/class/google_os_config_patch_deployment"/>
    <rdfs:range rdf:resource="http://www.w3.org/2001/XMLSchema#string"/>
  </owl:DatatypeProperty>
  <owl:DatatypeProperty rdf:about="http://example.org/onto/prop/google_os_config_patch_deployment_instance_name_prefixes">
    <rdfs:label>instance_name_prefixes</rdfs:label>
    <rdfs:comment>Targets VMs whose name starts with one of these prefixes. Similar to labels, this is another way to group
VMs when targeting configs, for example prefix="prod-".</rdfs:comment>
    <rdfs:domain rdf:resource="http://example.org/onto/class/google_os_config_patch_deployment"/>
    <rdfs:range rdf:resource="http://www.w3.org/2001/XMLSchema#string"/>
  </owl:DatatypeProperty>
  <owl:DatatypeProperty rdf:about="http://example.org/onto/prop/google_os_config_patch_deployment_instances">
    <rdfs:label>instances</rdfs:label>
    <rdfs:comment>Targets any of the VM instances specified. Instances are specified by their URI in the 'form zones/{{zone}}/instances/{{instance_name}}',
'projects/{{project_id}}/zones/{{zone}}/instances/{{instance_name}}', or
'https://www.googleapis.com/compute/v1/projects/{{project_id}}/zones/{{zone}}/instances/{{instance_name}}'</rdfs:comment>
    <rdfs:domain rdf:resource="http://example.org/onto/class/google_os_config_patch_deployment"/>
    <rdfs:range rdf:resource="http://www.w3.org/2001/XMLSchema#string"/>
  </owl:DatatypeProperty>
  <owl:DatatypeProperty rdf:about="http://example.org/onto/prop/google_os_config_patch_deployment_zones">
    <rdfs:label>zones</rdfs:label>
    <rdfs:comment>Targets VM instances in ANY of these zones. Leave empty to target VM instances in any zone.</rdfs:comment>
    <rdfs:domain rdf:resource="http://example.org/onto/class/google_os_config_patch_deployment"/>
    <rdfs:range rdf:resource="http://www.w3.org/2001/XMLSchema#string"/>
  </owl:DatatypeProperty>
  <owl:DatatypeProperty rdf:about="http://example.org/onto/prop/google_os_config_patch_deployment_labels">
    <rdfs:label>labels</rdfs:label>
    <rdfs:comment>Compute Engine instance labels that must be present for a VM instance to be targeted by this filter</rdfs:comment>
    <rdfs:domain rdf:resource="http://example.org/onto/class/google_os_config_patch_deployment"/>
    <rdfs:range rdf:resource="http://www.w3.org/2001/XMLSchema#string"/>
  </owl:DatatypeProperty>
  <owl:DatatypeProperty rdf:about="http://example.org/onto/prop/google_os_config_patch_deployment_execute_time">
    <rdfs:label>execute_time</rdfs:label>
    <rdfs:comment>The desired patch job execution time. A timestamp in RFC3339 UTC "Zulu" format,
accurate to nanoseconds. Example: "2014-10-02T15:01:23.045123456Z".</rdfs:comment>
    <rdfs:domain rdf:resource="http://example.org/onto/class/google_os_config_patch_deployment"/>
    <rdfs:range rdf:resource="http://www.w3.org/2001/XMLSchema#string"/>
  </owl:DatatypeProperty>
  <owl:DatatypeProperty rdf:about="http://example.org/onto/prop/google_os_config_patch_deployment_mig_instances_allowed">
    <rdfs:label>mig_instances_allowed</rdfs:label>
    <rdfs:comment>Allows the patch job to run on Managed instance groups (MIGs).</rdfs:comment>
    <rdfs:domain rdf:resource="http://example.org/onto/class/google_os_config_patch_deployment"/>
    <rdfs:range rdf:resource="http://www.w3.org/2001/XMLSchema#string"/>
  </owl:DatatypeProperty>
  <owl:DatatypeProperty rdf:about="http://example.org/onto/prop/google_os_config_patch_deployment_reboot_config">
    <rdfs:label>reboot_config</rdfs:label>
    <rdfs:comment>Post-patch reboot settings. Possible values: ["DEFAULT", "ALWAYS", "NEVER"]</rdfs:comment>
    <rdfs:domain rdf:resource="http://example.org/onto/class/google_os_config_patch_deployment"/>
    <rdfs:range rdf:resource="http://www.w3.org/2001/XMLSchema#string"/>
  </owl:DatatypeProperty>
  <owl:DatatypeProperty rdf:about="http://example.org/onto/prop/google_os_config_patch_deployment_excludes">
    <rdfs:label>excludes</rdfs:label>
    <rdfs:comment>List of packages to exclude from update. These packages will be excluded.</rdfs:comment>
    <rdfs:domain rdf:resource="http://example.org/onto/class/google_os_config_patch_deployment"/>
    <rdfs:range rdf:resource="http://www.w3.org/2001/XMLSchema#string"/>
  </owl:DatatypeProperty>
  <owl:DatatypeProperty rdf:about="http://example.org/onto/prop/google_os_config_patch_deployment_exclusive_packages">
    <rdfs:label>exclusive_packages</rdfs:label>
    <rdfs:comment>An exclusive list of packages to be updated. These are the only packages that will be updated.
If these packages are not installed, they will be ignored. This field cannot be specified with
any other patch configuration fields.</rdfs:comment>
    <rdfs:domain rdf:resource="http://example.org/onto/class/google_os_config_patch_deployment"/>
    <rdfs:range rdf:resource="http://www.w3.org/2001/XMLSchema#string"/>
  </owl:DatatypeProperty>
  <owl:DatatypeProperty rdf:about="http://example.org/onto/prop/google_os_config_patch_deployment_type">
    <rdfs:label>type</rdfs:label>
    <rdfs:comment>By changing the type to DIST, the patching is performed using apt-get dist-upgrade instead. Possible values: ["DIST", "UPGRADE"]</rdfs:comment>
    <rdfs:domain rdf:resource="http://example.org/onto/class/google_os_config_patch_deployment"/>
    <rdfs:range rdf:resource="http://www.w3.org/2001/XMLSchema#string"/>
  </owl:DatatypeProperty>
  <owl:DatatypeProperty rdf:about="http://example.org/onto/prop/google_os_config_patch_deployment_enabled">
    <rdfs:label>enabled</rdfs:label>
    <rdfs:comment>goo update settings. Use this setting to override the default goo patch rules.</rdfs:comment>
    <rdfs:domain rdf:resource="http://example.org/onto/class/google_os_config_patch_deployment"/>
    <rdfs:range rdf:resource="http://www.w3.org/2001/XMLSchema#string"/>
  </owl:DatatypeProperty>
  <owl:DatatypeProperty rdf:about="http://example.org/onto/prop/google_os_config_patch_deployment_allowed_success_codes">
    <rdfs:label>allowed_success_codes</rdfs:label>
    <rdfs:comment>Defaults to [0]. A list of possible return values that the execution can return to indicate a success.</rdfs:comment>
    <rdfs:domain rdf:resource="http://example.org/onto/class/google_os_config_patch_deployment"/>
    <rdfs:range rdf:resource="http://www.w3.org/2001/XMLSchema#string"/>
  </owl:DatatypeProperty>
  <owl:DatatypeProperty rdf:about="http://example.org/onto/prop/google_os_config_patch_deployment_interpreter">
    <rdfs:label>interpreter</rdfs:label>
    <rdfs:comment>The script interpreter to use to run the script. If no interpreter is specified the script will
be executed directly, which will likely only succeed for scripts with shebang lines. Possible values: ["SHELL", "POWERSHELL"]</rdfs:comment>
    <rdfs:domain rdf:resource="http://example.org/onto/class/google_os_config_patch_deployment"/>
    <rdfs:range rdf:resource="http://www.w3.org/2001/XMLSchema#string"/>
  </owl:DatatypeProperty>
  <owl:DatatypeProperty rdf:about="http://example.org/onto/prop/google_os_config_patch_deployment_local_path">
    <rdfs:label>local_path</rdfs:label>
    <rdfs:comment>An absolute path to the executable on the VM.</rdfs:comment>
    <rdfs:domain rdf:resource="http://example.org/onto/class/google_os_config_patch_deployment"/>
    <rdfs:range rdf:resource="http://www.w3.org/2001/XMLSchema#string"/>
  </owl:DatatypeProperty>
  <owl:DatatypeProperty rdf:about="http://example.org/onto/prop/google_os_config_patch_deployment_bucket">
    <rdfs:label>bucket</rdfs:label>
    <rdfs:comment>Bucket of the Cloud Storage object.</rdfs:comment>
    <rdfs:domain rdf:resource="http://example.org/onto/class/google_os_config_patch_deployment"/>
    <rdfs:range rdf:resource="http://www.w3.org/2001/XMLSchema#string"/>
  </owl:DatatypeProperty>
  <owl:DatatypeProperty rdf:about="http://example.org/onto/prop/google_os_config_patch_deployment_generation_number">
    <rdfs:label>generation_number</rdfs:label>
    <rdfs:comment>Generation number of the Cloud Storage object. This is used to ensure that the ExecStep specified by this PatchJob does not change.</rdfs:comment>
    <rdfs:domain rdf:resource="http://example.org/onto/class/google_os_config_patch_deployment"/>
    <rdfs:range rdf:resource="http://www.w3.org/2001/XMLSchema#string"/>
  </owl:DatatypeProperty>
  <owl:DatatypeProperty rdf:about="http://example.org/onto/prop/google_os_config_patch_deployment_object">
    <rdfs:label>object</rdfs:label>
    <rdfs:comment>Name of the Cloud Storage object.</rdfs:comment>
    <rdfs:domain rdf:resource="http://example.org/onto/class/google_os_config_patch_deployment"/>
    <rdfs:range rdf:resource="http://www.w3.org/2001/XMLSchema#string"/>
  </owl:DatatypeProperty>
  <owl:DatatypeProperty rdf:about="http://example.org/onto/prop/google_os_config_patch_deployment_allowed_success_codes">
    <rdfs:label>allowed_success_codes</rdfs:label>
    <rdfs:comment>Defaults to [0]. A list of possible return values that the execution can return to indicate a success.</rdfs:comment>
    <rdfs:domain rdf:resource="http://example.org/onto/class/google_os_config_patch_deployment"/>
    <rdfs:range rdf:resource="http://www.w3.org/2001/XMLSchema#string"/>
  </owl:DatatypeProperty>
  <owl:DatatypeProperty rdf:about="http://example.org/onto/prop/google_os_config_patch_deployment_interpreter">
    <rdfs:label>interpreter</rdfs:label>
    <rdfs:comment>The script interpreter to use to run the script. If no interpreter is specified the script will
be executed directly, which will likely only succeed for scripts with shebang lines. Possible values: ["SHELL", "POWERSHELL"]</rdfs:comment>
    <rdfs:domain rdf:resource="http://example.org/onto/class/google_os_config_patch_deployment"/>
    <rdfs:range rdf:resource="http://www.w3.org/2001/XMLSchema#string"/>
  </owl:DatatypeProperty>
  <owl:DatatypeProperty rdf:about="http://example.org/onto/prop/google_os_config_patch_deployment_local_path">
    <rdfs:label>local_path</rdfs:label>
    <rdfs:comment>An absolute path to the executable on the VM.</rdfs:comment>
    <rdfs:domain rdf:resource="http://example.org/onto/class/google_os_config_patch_deployment"/>
    <rdfs:range rdf:resource="http://www.w3.org/2001/XMLSchema#string"/>
  </owl:DatatypeProperty>
  <owl:DatatypeProperty rdf:about="http://example.org/onto/prop/google_os_config_patch_deployment_bucket">
    <rdfs:label>bucket</rdfs:label>
    <rdfs:comment>Bucket of the Cloud Storage object.</rdfs:comment>
    <rdfs:domain rdf:resource="http://example.org/onto/class/google_os_config_patch_deployment"/>
    <rdfs:range rdf:resource="http://www.w3.org/2001/XMLSchema#string"/>
  </owl:DatatypeProperty>
  <owl:DatatypeProperty rdf:about="http://example.org/onto/prop/google_os_config_patch_deployment_generation_number">
    <rdfs:label>generation_number</rdfs:label>
    <rdfs:comment>Generation number of the Cloud Storage object. This is used to ensure that the ExecStep specified by this PatchJob does not change.</rdfs:comment>
    <rdfs:domain rdf:resource="http://example.org/onto/class/google_os_config_patch_deployment"/>
    <rdfs:range rdf:resource="http://www.w3.org/2001/XMLSchema#string"/>
  </owl:DatatypeProperty>
  <owl:DatatypeProperty rdf:about="http://example.org/onto/prop/google_os_config_patch_deployment_object">
    <rdfs:label>object</rdfs:label>
    <rdfs:comment>Name of the Cloud Storage object.</rdfs:comment>
    <rdfs:domain rdf:resource="http://example.org/onto/class/google_os_config_patch_deployment"/>
    <rdfs:range rdf:resource="http://www.w3.org/2001/XMLSchema#string"/>
  </owl:DatatypeProperty>
  <owl:DatatypeProperty rdf:about="http://example.org/onto/prop/google_os_config_patch_deployment_allowed_success_codes">
    <rdfs:label>allowed_success_codes</rdfs:label>
    <rdfs:comment>Defaults to [0]. A list of possible return values that the execution can return to indicate a success.</rdfs:comment>
    <rdfs:domain rdf:resource="http://example.org/onto/class/google_os_config_patch_deployment"/>
    <rdfs:range rdf:resource="http://www.w3.org/2001/XMLSchema#string"/>
  </owl:DatatypeProperty>
  <owl:DatatypeProperty rdf:about="http://example.org/onto/prop/google_os_config_patch_deployment_interpreter">
    <rdfs:label>interpreter</rdfs:label>
    <rdfs:comment>The script interpreter to use to run the script. If no interpreter is specified the script will
be executed directly, which will likely only succeed for scripts with shebang lines. Possible values: ["SHELL", "POWERSHELL"]</rdfs:comment>
    <rdfs:domain rdf:resource="http://example.org/onto/class/google_os_config_patch_deployment"/>
    <rdfs:range rdf:resource="http://www.w3.org/2001/XMLSchema#string"/>
  </owl:DatatypeProperty>
  <owl:DatatypeProperty rdf:about="http://example.org/onto/prop/google_os_config_patch_deployment_local_path">
    <rdfs:label>local_path</rdfs:label>
    <rdfs:comment>An absolute path to the executable on the VM.</rdfs:comment>
    <rdfs:domain rdf:resource="http://example.org/onto/class/google_os_config_patch_deployment"/>
    <rdfs:range rdf:resource="http://www.w3.org/2001/XMLSchema#string"/>
  </owl:DatatypeProperty>
  <owl:DatatypeProperty rdf:about="http://example.org/onto/prop/google_os_config_patch_deployment_bucket">
    <rdfs:label>bucket</rdfs:label>
    <rdfs:comment>Bucket of the Cloud Storage object.</rdfs:comment>
    <rdfs:domain rdf:resource="http://example.org/onto/class/google_os_config_patch_deployment"/>
    <rdfs:range rdf:resource="http://www.w3.org/2001/XMLSchema#string"/>
  </owl:DatatypeProperty>
  <owl:DatatypeProperty rdf:about="http://example.org/onto/prop/google_os_config_patch_deployment_generation_number">
    <rdfs:label>generation_number</rdfs:label>
    <rdfs:comment>Generation number of the Cloud Storage object. This is used to ensure that the ExecStep specified by this PatchJob does not change.</rdfs:comment>
    <rdfs:domain rdf:resource="http://example.org/onto/class/google_os_config_patch_deployment"/>
    <rdfs:range rdf:resource="http://www.w3.org/2001/XMLSchema#string"/>
  </owl:DatatypeProperty>
  <owl:DatatypeProperty rdf:about="http://example.org/onto/prop/google_os_config_patch_deployment_object">
    <rdfs:label>object</rdfs:label>
    <rdfs:comment>Name of the Cloud Storage object.</rdfs:comment>
    <rdfs:domain rdf:resource="http://example.org/onto/class/google_os_config_patch_deployment"/>
    <rdfs:range rdf:resource="http://www.w3.org/2001/XMLSchema#string"/>
  </owl:DatatypeProperty>
  <owl:DatatypeProperty rdf:about="http://example.org/onto/prop/google_os_config_patch_deployment_allowed_success_codes">
    <rdfs:label>allowed_success_codes</rdfs:label>
    <rdfs:comment>Defaults to [0]. A list of possible return values that the execution can return to indicate a success.</rdfs:comment>
    <rdfs:domain rdf:resource="http://example.org/onto/class/google_os_config_patch_deployment"/>
    <rdfs:range rdf:resource="http://www.w3.org/2001/XMLSchema#string"/>
  </owl:DatatypeProperty>
  <owl:DatatypeProperty rdf:about="http://example.org/onto/prop/google_os_config_patch_deployment_interpreter">
    <rdfs:label>interpreter</rdfs:label>
    <rdfs:comment>The script interpreter to use to run the script. If no interpreter is specified the script will
be executed directly, which will likely only succeed for scripts with shebang lines. Possible values: ["SHELL", "POWERSHELL"]</rdfs:comment>
    <rdfs:domain rdf:resource="http://example.org/onto/class/google_os_config_patch_deployment"/>
    <rdfs:range rdf:resource="http://www.w3.org/2001/XMLSchema#string"/>
  </owl:DatatypeProperty>
  <owl:DatatypeProperty rdf:about="http://example.org/onto/prop/google_os_config_patch_deployment_local_path">
    <rdfs:label>local_path</rdfs:label>
    <rdfs:comment>An absolute path to the executable on the VM.</rdfs:comment>
    <rdfs:domain rdf:resource="http://example.org/onto/class/google_os_config_patch_deployment"/>
    <rdfs:range rdf:resource="http://www.w3.org/2001/XMLSchema#string"/>
  </owl:DatatypeProperty>
  <owl:DatatypeProperty rdf:about="http://example.org/onto/prop/google_os_config_patch_deployment_bucket">
    <rdfs:label>bucket</rdfs:label>
    <rdfs:comment>Bucket of the Cloud Storage object.</rdfs:comment>
    <rdfs:domain rdf:resource="http://example.org/onto/class/google_os_config_patch_deployment"/>
    <rdfs:range rdf:resource="http://www.w3.org/2001/XMLSchema#string"/>
  </owl:DatatypeProperty>
  <owl:DatatypeProperty rdf:about="http://example.org/onto/prop/google_os_config_patch_deployment_generation_number">
    <rdfs:label>generation_number</rdfs:label>
    <rdfs:comment>Generation number of the Cloud Storage object. This is used to ensure that the ExecStep specified by this PatchJob does not change.</rdfs:comment>
    <rdfs:domain rdf:resource="http://example.org/onto/class/google_os_config_patch_deployment"/>
    <rdfs:range rdf:resource="http://www.w3.org/2001/XMLSchema#string"/>
  </owl:DatatypeProperty>
  <owl:DatatypeProperty rdf:about="http://example.org/onto/prop/google_os_config_patch_deployment_object">
    <rdfs:label>object</rdfs:label>
    <rdfs:comment>Name of the Cloud Storage object.</rdfs:comment>
    <rdfs:domain rdf:resource="http://example.org/onto/class/google_os_config_patch_deployment"/>
    <rdfs:range rdf:resource="http://www.w3.org/2001/XMLSchema#string"/>
  </owl:DatatypeProperty>
  <owl:DatatypeProperty rdf:about="http://example.org/onto/prop/google_os_config_patch_deployment_classifications">
    <rdfs:label>classifications</rdfs:label>
    <rdfs:comment>Only apply updates of these windows update classifications. If empty, all updates are applied. Possible values: ["CRITICAL", "SECURITY", "DEFINITION", "DRIVER", "FEATURE_PACK", "SERVICE_PACK", "TOOL", "UPDATE_ROLLUP", "UPDATE"]</rdfs:comment>
    <rdfs:domain rdf:resource="http://example.org/onto/class/google_os_config_patch_deployment"/>
    <rdfs:range rdf:resource="http://www.w3.org/2001/XMLSchema#string"/>
  </owl:DatatypeProperty>
  <owl:DatatypeProperty rdf:about="http://example.org/onto/prop/google_os_config_patch_deployment_excludes">
    <rdfs:label>excludes</rdfs:label>
    <rdfs:comment>List of KBs to exclude from update.</rdfs:comment>
    <rdfs:domain rdf:resource="http://example.org/onto/class/google_os_config_patch_deployment"/>
    <rdfs:range rdf:resource="http://www.w3.org/2001/XMLSchema#string"/>
  </owl:DatatypeProperty>
  <owl:DatatypeProperty rdf:about="http://example.org/onto/prop/google_os_config_patch_deployment_exclusive_patches">
    <rdfs:label>exclusive_patches</rdfs:label>
    <rdfs:comment>An exclusive list of kbs to be updated. These are the only patches that will be updated.
This field must not be used with other patch configurations.</rdfs:comment>
    <rdfs:domain rdf:resource="http://example.org/onto/class/google_os_config_patch_deployment"/>
    <rdfs:range rdf:resource="http://www.w3.org/2001/XMLSchema#string"/>
  </owl:DatatypeProperty>
  <owl:DatatypeProperty rdf:about="http://example.org/onto/prop/google_os_config_patch_deployment_excludes">
    <rdfs:label>excludes</rdfs:label>
    <rdfs:comment>List of packages to exclude from update. These packages will be excluded.</rdfs:comment>
    <rdfs:domain rdf:resource="http://example.org/onto/class/google_os_config_patch_deployment"/>
    <rdfs:range rdf:resource="http://www.w3.org/2001/XMLSchema#string"/>
  </owl:DatatypeProperty>
  <owl:DatatypeProperty rdf:about="http://example.org/onto/prop/google_os_config_patch_deployment_exclusive_packages">
    <rdfs:label>exclusive_packages</rdfs:label>
    <rdfs:comment>An exclusive list of packages to be updated. These are the only packages that will be updated.
If these packages are not installed, they will be ignored. This field cannot be specified with
any other patch configuration fields.</rdfs:comment>
    <rdfs:domain rdf:resource="http://example.org/onto/class/google_os_config_patch_deployment"/>
    <rdfs:range rdf:resource="http://www.w3.org/2001/XMLSchema#string"/>
  </owl:DatatypeProperty>
  <owl:DatatypeProperty rdf:about="http://example.org/onto/prop/google_os_config_patch_deployment_minimal">
    <rdfs:label>minimal</rdfs:label>
    <rdfs:comment>Will cause patch to run yum update-minimal instead.</rdfs:comment>
    <rdfs:domain rdf:resource="http://example.org/onto/class/google_os_config_patch_deployment"/>
    <rdfs:range rdf:resource="http://www.w3.org/2001/XMLSchema#string"/>
  </owl:DatatypeProperty>
  <owl:DatatypeProperty rdf:about="http://example.org/onto/prop/google_os_config_patch_deployment_security">
    <rdfs:label>security</rdfs:label>
    <rdfs:comment>Adds the --security flag to yum update. Not supported on all platforms.</rdfs:comment>
    <rdfs:domain rdf:resource="http://example.org/onto/class/google_os_config_patch_deployment"/>
    <rdfs:range rdf:resource="http://www.w3.org/2001/XMLSchema#string"/>
  </owl:DatatypeProperty>
  <owl:DatatypeProperty rdf:about="http://example.org/onto/prop/google_os_config_patch_deployment_categories">
    <rdfs:label>categories</rdfs:label>
    <rdfs:comment>Install only patches with these categories. Common categories include security, recommended, and feature.</rdfs:comment>
    <rdfs:domain rdf:resource="http://example.org/onto/class/google_os_config_patch_deployment"/>
    <rdfs:range rdf:resource="http://www.w3.org/2001/XMLSchema#string"/>
  </owl:DatatypeProperty>
  <owl:DatatypeProperty rdf:about="http://example.org/onto/prop/google_os_config_patch_deployment_excludes">
    <rdfs:label>excludes</rdfs:label>
    <rdfs:comment>List of packages to exclude from update.</rdfs:comment>
    <rdfs:domain rdf:resource="http://example.org/onto/class/google_os_config_patch_deployment"/>
    <rdfs:range rdf:resource="http://www.w3.org/2001/XMLSchema#string"/>
  </owl:DatatypeProperty>
  <owl:DatatypeProperty rdf:about="http://example.org/onto/prop/google_os_config_patch_deployment_exclusive_patches">
    <rdfs:label>exclusive_patches</rdfs:label>
    <rdfs:comment>An exclusive list of patches to be updated. These are the only patches that will be installed using 'zypper patch patch:' command.
This field must not be used with any other patch configuration fields.</rdfs:comment>
    <rdfs:domain rdf:resource="http://example.org/onto/class/google_os_config_patch_deployment"/>
    <rdfs:range rdf:resource="http://www.w3.org/2001/XMLSchema#string"/>
  </owl:DatatypeProperty>
  <owl:DatatypeProperty rdf:about="http://example.org/onto/prop/google_os_config_patch_deployment_severities">
    <rdfs:label>severities</rdfs:label>
    <rdfs:comment>Install only patches with these severities. Common severities include critical, important, moderate, and low.</rdfs:comment>
    <rdfs:domain rdf:resource="http://example.org/onto/class/google_os_config_patch_deployment"/>
    <rdfs:range rdf:resource="http://www.w3.org/2001/XMLSchema#string"/>
  </owl:DatatypeProperty>
  <owl:DatatypeProperty rdf:about="http://example.org/onto/prop/google_os_config_patch_deployment_with_optional">
    <rdfs:label>with_optional</rdfs:label>
    <rdfs:comment>Adds the --with-optional flag to zypper patch.</rdfs:comment>
    <rdfs:domain rdf:resource="http://example.org/onto/class/google_os_config_patch_deployment"/>
    <rdfs:range rdf:resource="http://www.w3.org/2001/XMLSchema#string"/>
  </owl:DatatypeProperty>
  <owl:DatatypeProperty rdf:about="http://example.org/onto/prop/google_os_config_patch_deployment_with_update">
    <rdfs:label>with_update</rdfs:label>
    <rdfs:comment>Adds the --with-update flag, to zypper patch.</rdfs:comment>
    <rdfs:domain rdf:resource="http://example.org/onto/class/google_os_config_patch_deployment"/>
    <rdfs:range rdf:resource="http://www.w3.org/2001/XMLSchema#string"/>
  </owl:DatatypeProperty>
  <owl:DatatypeProperty rdf:about="http://example.org/onto/prop/google_os_config_patch_deployment_end_time">
    <rdfs:label>end_time</rdfs:label>
    <rdfs:comment>The end time at which a recurring patch deployment schedule is no longer active.
A timestamp in RFC3339 UTC "Zulu" format, accurate to nanoseconds. Example: "2014-10-02T15:01:23.045123456Z".</rdfs:comment>
    <rdfs:domain rdf:resource="http://example.org/onto/class/google_os_config_patch_deployment"/>
    <rdfs:range rdf:resource="http://www.w3.org/2001/XMLSchema#string"/>
  </owl:DatatypeProperty>
  <owl:DatatypeProperty rdf:about="http://example.org/onto/prop/google_os_config_patch_deployment_last_execute_time">
    <rdfs:label>last_execute_time</rdfs:label>
    <rdfs:comment>The time the last patch job ran successfully.
A timestamp in RFC3339 UTC "Zulu" format, accurate to nanoseconds. Example: "2014-10-02T15:01:23.045123456Z".</rdfs:comment>
    <rdfs:domain rdf:resource="http://example.org/onto/class/google_os_config_patch_deployment"/>
    <rdfs:range rdf:resource="http://www.w3.org/2001/XMLSchema#string"/>
  </owl:DatatypeProperty>
  <owl:DatatypeProperty rdf:about="http://example.org/onto/prop/google_os_config_patch_deployment_next_execute_time">
    <rdfs:label>next_execute_time</rdfs:label>
    <rdfs:comment>The time the next patch job is scheduled to run.
A timestamp in RFC3339 UTC "Zulu" format, accurate to nanoseconds. Example: "2014-10-02T15:01:23.045123456Z".</rdfs:comment>
    <rdfs:domain rdf:resource="http://example.org/onto/class/google_os_config_patch_deployment"/>
    <rdfs:range rdf:resource="http://www.w3.org/2001/XMLSchema#string"/>
  </owl:DatatypeProperty>
  <owl:DatatypeProperty rdf:about="http://example.org/onto/prop/google_os_config_patch_deployment_start_time">
    <rdfs:label>start_time</rdfs:label>
    <rdfs:comment>The time that the recurring schedule becomes effective. Defaults to createTime of the patch deployment.
A timestamp in RFC3339 UTC "Zulu" format, accurate to nanoseconds. Example: "2014-10-02T15:01:23.045123456Z".</rdfs:comment>
    <rdfs:domain rdf:resource="http://example.org/onto/class/google_os_config_patch_deployment"/>
    <rdfs:range rdf:resource="http://www.w3.org/2001/XMLSchema#string"/>
  </owl:DatatypeProperty>
  <owl:DatatypeProperty rdf:about="http://example.org/onto/prop/google_os_config_patch_deployment_month_day">
    <rdfs:label>month_day</rdfs:label>
    <rdfs:comment>One day of the month. 1-31 indicates the 1st to the 31st day. -1 indicates the last day of the month.
Months without the target day will be skipped. For example, a schedule to run "every month on the 31st"
will not run in February, April, June, etc.</rdfs:comment>
    <rdfs:domain rdf:resource="http://example.org/onto/class/google_os_config_patch_deployment"/>
    <rdfs:range rdf:resource="http://www.w3.org/2001/XMLSchema#string"/>
  </owl:DatatypeProperty>
  <owl:DatatypeProperty rdf:about="http://example.org/onto/prop/google_os_config_patch_deployment_day_of_week">
    <rdfs:label>day_of_week</rdfs:label>
    <rdfs:comment>A day of the week. Possible values: ["MONDAY", "TUESDAY", "WEDNESDAY", "THURSDAY", "FRIDAY", "SATURDAY", "SUNDAY"]</rdfs:comment>
    <rdfs:domain rdf:resource="http://example.org/onto/class/google_os_config_patch_deployment"/>
    <rdfs:range rdf:resource="http://www.w3.org/2001/XMLSchema#string"/>
  </owl:DatatypeProperty>
  <owl:DatatypeProperty rdf:about="http://example.org/onto/prop/google_os_config_patch_deployment_day_offset">
    <rdfs:label>day_offset</rdfs:label>
    <rdfs:comment>Represents the number of days before or after the given week day of month that the patch deployment is scheduled for.</rdfs:comment>
    <rdfs:domain rdf:resource="http://example.org/onto/class/google_os_config_patch_deployment"/>
    <rdfs:range rdf:resource="http://www.w3.org/2001/XMLSchema#string"/>
  </owl:DatatypeProperty>
  <owl:DatatypeProperty rdf:about="http://example.org/onto/prop/google_os_config_patch_deployment_week_ordinal">
    <rdfs:label>week_ordinal</rdfs:label>
    <rdfs:comment>Week number in a month. 1-4 indicates the 1st to 4th week of the month. -1 indicates the last week of the month.</rdfs:comment>
    <rdfs:domain rdf:resource="http://example.org/onto/class/google_os_config_patch_deployment"/>
    <rdfs:range rdf:resource="http://www.w3.org/2001/XMLSchema#string"/>
  </owl:DatatypeProperty>
  <owl:DatatypeProperty rdf:about="http://example.org/onto/prop/google_os_config_patch_deployment_hours">
    <rdfs:label>hours</rdfs:label>
    <rdfs:comment>Hours of day in 24 hour format. Should be from 0 to 23.
An API may choose to allow the value "24:00:00" for scenarios like business closing time.</rdfs:comment>
    <rdfs:domain rdf:resource="http://example.org/onto/class/google_os_config_patch_deployment"/>
    <rdfs:range rdf:resource="http://www.w3.org/2001/XMLSchema#string"/>
  </owl:DatatypeProperty>
  <owl:DatatypeProperty rdf:about="http://example.org/onto/prop/google_os_config_patch_deployment_minutes">
    <rdfs:label>minutes</rdfs:label>
    <rdfs:comment>Minutes of hour of day. Must be from 0 to 59.</rdfs:comment>
    <rdfs:domain rdf:resource="http://example.org/onto/class/google_os_config_patch_deployment"/>
    <rdfs:range rdf:resource="http://www.w3.org/2001/XMLSchema#string"/>
  </owl:DatatypeProperty>
  <owl:DatatypeProperty rdf:about="http://example.org/onto/prop/google_os_config_patch_deployment_nanos">
    <rdfs:label>nanos</rdfs:label>
    <rdfs:comment>Fractions of seconds in nanoseconds. Must be from 0 to 999,999,999.</rdfs:comment>
    <rdfs:domain rdf:resource="http://example.org/onto/class/google_os_config_patch_deployment"/>
    <rdfs:range rdf:resource="http://www.w3.org/2001/XMLSchema#string"/>
  </owl:DatatypeProperty>
  <owl:DatatypeProperty rdf:about="http://example.org/onto/prop/google_os_config_patch_deployment_seconds">
    <rdfs:label>seconds</rdfs:label>
    <rdfs:comment>Seconds of minutes of the time. Must normally be from 0 to 59. An API may allow the value 60 if it allows leap-seconds.</rdfs:comment>
    <rdfs:domain rdf:resource="http://example.org/onto/class/google_os_config_patch_deployment"/>
    <rdfs:range rdf:resource="http://www.w3.org/2001/XMLSchema#string"/>
  </owl:DatatypeProperty>
  <owl:DatatypeProperty rdf:about="http://example.org/onto/prop/google_os_config_patch_deployment_id">
    <rdfs:label>id</rdfs:label>
    <rdfs:comment>IANA Time Zone Database time zone, e.g. "America/New_York".</rdfs:comment>
    <rdfs:domain rdf:resource="http://example.org/onto/class/google_os_config_patch_deployment"/>
    <rdfs:range rdf:resource="http://www.w3.org/2001/XMLSchema#string"/>
  </owl:DatatypeProperty>
  <owl:DatatypeProperty rdf:about="http://example.org/onto/prop/google_os_config_patch_deployment_version">
    <rdfs:label>version</rdfs:label>
    <rdfs:comment>IANA Time Zone Database version number, e.g. "2019a".</rdfs:comment>
    <rdfs:domain rdf:resource="http://example.org/onto/class/google_os_config_patch_deployment"/>
    <rdfs:range rdf:resource="http://www.w3.org/2001/XMLSchema#string"/>
  </owl:DatatypeProperty>
  <owl:DatatypeProperty rdf:about="http://example.org/onto/prop/google_os_config_patch_deployment_day_of_week">
    <rdfs:label>day_of_week</rdfs:label>
    <rdfs:comment>IANA Time Zone Database time zone, e.g. "America/New_York". Possible values: ["MONDAY", "TUESDAY", "WEDNESDAY", "THURSDAY", "FRIDAY", "SATURDAY", "SUNDAY"]</rdfs:comment>
    <rdfs:domain rdf:resource="http://example.org/onto/class/google_os_config_patch_deployment"/>
    <rdfs:range rdf:resource="http://www.w3.org/2001/XMLSchema#string"/>
  </owl:DatatypeProperty>
  <owl:DatatypeProperty rdf:about="http://example.org/onto/prop/google_os_config_patch_deployment_mode">
    <rdfs:label>mode</rdfs:label>
    <rdfs:comment>Mode of the patch rollout. Possible values: ["ZONE_BY_ZONE", "CONCURRENT_ZONES"]</rdfs:comment>
    <rdfs:domain rdf:resource="http://example.org/onto/class/google_os_config_patch_deployment"/>
    <rdfs:range rdf:resource="http://www.w3.org/2001/XMLSchema#string"/>
  </owl:DatatypeProperty>
  <owl:DatatypeProperty rdf:about="http://example.org/onto/prop/google_os_config_patch_deployment_fixed">
    <rdfs:label>fixed</rdfs:label>
    <rdfs:comment>Specifies a fixed value.</rdfs:comment>
    <rdfs:domain rdf:resource="http://example.org/onto/class/google_os_config_patch_deployment"/>
    <rdfs:range rdf:resource="http://www.w3.org/2001/XMLSchema#string"/>
  </owl:DatatypeProperty>
  <owl:DatatypeProperty rdf:about="http://example.org/onto/prop/google_os_config_patch_deployment_percentage">
    <rdfs:label>percentage</rdfs:label>
    <rdfs:comment>Specifies the relative value defined as a percentage, which will be multiplied by a reference value.</rdfs:comment>
    <rdfs:domain rdf:resource="http://example.org/onto/class/google_os_config_patch_deployment"/>
    <rdfs:range rdf:resource="http://www.w3.org/2001/XMLSchema#string"/>
  </owl:DatatypeProperty>
  <owl:DatatypeProperty rdf:about="http://example.org/onto/prop/google_os_config_patch_deployment_create">
    <rdfs:label>create</rdfs:label>
    <rdfs:domain rdf:resource="http://example.org/onto/class/google_os_config_patch_deployment"/>
    <rdfs:range rdf:resource="http://www.w3.org/2001/XMLSchema#string"/>
  </owl:DatatypeProperty>
  <owl:DatatypeProperty rdf:about="http://example.org/onto/prop/google_os_config_patch_deployment_delete">
    <rdfs:label>delete</rdfs:label>
    <rdfs:domain rdf:resource="http://example.org/onto/class/google_os_config_patch_deployment"/>
    <rdfs:range rdf:resource="http://www.w3.org/2001/XMLSchema#string"/>
  </owl:DatatypeProperty>
</rdf:RDF>
