<?xml version="1.0" encoding="UTF-8"?>
<rdf:RDF
  xmlns:rdf="http://www.w3.org/1999/02/22-rdf-syntax-ns#"
  xmlns:rdfs="http://www.w3.org/2000/01/rdf-schema#"
  xmlns:owl="http://www.w3.org/2002/07/owl#"
  xmlns:xsd="http://www.w3.org/2001/XMLSchema#"
  xml:base="http://example.org/onto/">
  <owl:Class rdf:about="http://example.org/onto/class/google_privateca_ca_pool">
    <rdfs:label>google_privateca_ca_pool</rdfs:label>
    <rdfs:comment>#
#     ***     AUTO GENERATED CODE    ***    Type: MMv1     ***
#
# ----------------------------------------------------------------------------
#
#     This code is generated by Magic Modules using the following:
#
#     Configuration: https:#github.com/GoogleCloudPlatform/magic-modules/tree/main/mmv1/products/privateca/CaPool.yaml
#     Template:      https:#github.com/GoogleCloudPlatform/magic-modules/tree/main/mmv1/templates/terraform/resource.html.markdown.tmpl
#
#     DO NOT EDIT this file directly. Any changes made to this file will be
#     overwritten during the next generation cycle.
#
# ----------------------------------------------------------------------------
subcategory: "Certificate Authority Service"
description: |-
  A CaPool represents a group of CertificateAuthorities that form a trust anchor.
---</rdfs:comment>
  </owl:Class>
  <owl:DatatypeProperty rdf:about="http://example.org/onto/prop/google_privateca_ca_pool_effective_labels">
    <rdfs:label>effective_labels</rdfs:label>
    <rdfs:comment>All of labels (key/value pairs) present on the resource in GCP, including the labels configured through Terraform, other clients and services.</rdfs:comment>
    <rdfs:domain rdf:resource="http://example.org/onto/class/google_privateca_ca_pool"/>
    <rdfs:range rdf:resource="http://www.w3.org/2001/XMLSchema#string"/>
  </owl:DatatypeProperty>
  <owl:DatatypeProperty rdf:about="http://example.org/onto/prop/google_privateca_ca_pool_id">
    <rdfs:label>id</rdfs:label>
    <rdfs:domain rdf:resource="http://example.org/onto/class/google_privateca_ca_pool"/>
    <rdfs:range rdf:resource="http://www.w3.org/2001/XMLSchema#string"/>
  </owl:DatatypeProperty>
  <owl:DatatypeProperty rdf:about="http://example.org/onto/prop/google_privateca_ca_pool_labels">
    <rdfs:label>labels</rdfs:label>
    <rdfs:comment>Labels with user-defined metadata.

An object containing a list of "key": value pairs. Example: { "name": "wrench", "mass":
"1.3kg", "count": "3" }.


**Note**: This field is non-authoritative, and will only manage the labels present in your configuration.
Please refer to the field 'effective_labels' for all of the labels present on the resource.</rdfs:comment>
    <rdfs:domain rdf:resource="http://example.org/onto/class/google_privateca_ca_pool"/>
    <rdfs:range rdf:resource="http://www.w3.org/2001/XMLSchema#string"/>
  </owl:DatatypeProperty>
  <owl:DatatypeProperty rdf:about="http://example.org/onto/prop/google_privateca_ca_pool_location">
    <rdfs:label>location</rdfs:label>
    <rdfs:comment>Location of the CaPool. A full list of valid locations can be found by
running 'gcloud privateca locations list'.</rdfs:comment>
    <rdfs:domain rdf:resource="http://example.org/onto/class/google_privateca_ca_pool"/>
    <rdfs:range rdf:resource="http://www.w3.org/2001/XMLSchema#string"/>
  </owl:DatatypeProperty>
  <owl:DatatypeProperty rdf:about="http://example.org/onto/prop/google_privateca_ca_pool_name">
    <rdfs:label>name</rdfs:label>
    <rdfs:comment>The name for this CaPool.</rdfs:comment>
    <rdfs:domain rdf:resource="http://example.org/onto/class/google_privateca_ca_pool"/>
    <rdfs:range rdf:resource="http://www.w3.org/2001/XMLSchema#string"/>
  </owl:DatatypeProperty>
  <owl:DatatypeProperty rdf:about="http://example.org/onto/prop/google_privateca_ca_pool_project">
    <rdfs:label>project</rdfs:label>
    <rdfs:domain rdf:resource="http://example.org/onto/class/google_privateca_ca_pool"/>
    <rdfs:range rdf:resource="http://www.w3.org/2001/XMLSchema#string"/>
  </owl:DatatypeProperty>
  <owl:DatatypeProperty rdf:about="http://example.org/onto/prop/google_privateca_ca_pool_terraform_labels">
    <rdfs:label>terraform_labels</rdfs:label>
    <rdfs:comment>The combination of labels configured directly on the resource
 and default labels configured on the provider.</rdfs:comment>
    <rdfs:domain rdf:resource="http://example.org/onto/class/google_privateca_ca_pool"/>
    <rdfs:range rdf:resource="http://www.w3.org/2001/XMLSchema#string"/>
  </owl:DatatypeProperty>
  <owl:DatatypeProperty rdf:about="http://example.org/onto/prop/google_privateca_ca_pool_tier">
    <rdfs:label>tier</rdfs:label>
    <rdfs:comment>The Tier of this CaPool. Possible values: ["ENTERPRISE", "DEVOPS"]</rdfs:comment>
    <rdfs:domain rdf:resource="http://example.org/onto/class/google_privateca_ca_pool"/>
    <rdfs:range rdf:resource="http://www.w3.org/2001/XMLSchema#string"/>
  </owl:DatatypeProperty>
  <owl:DatatypeProperty rdf:about="http://example.org/onto/prop/google_privateca_ca_pool_cloud_kms_key">
    <rdfs:label>cloud_kms_key</rdfs:label>
    <rdfs:comment>The resource name for an existing Cloud KMS key in the format
'projects/*/locations/*/keyRings/*/cryptoKeys/*'.</rdfs:comment>
    <rdfs:domain rdf:resource="http://example.org/onto/class/google_privateca_ca_pool"/>
    <rdfs:range rdf:resource="http://www.w3.org/2001/XMLSchema#string"/>
  </owl:DatatypeProperty>
  <owl:DatatypeProperty rdf:about="http://example.org/onto/prop/google_privateca_ca_pool_backdate_duration">
    <rdfs:label>backdate_duration</rdfs:label>
    <rdfs:comment>The duration to backdate all certificates issued from this CaPool. If not set, the
certificates will be issued with a not_before_time of the issuance time (i.e. the current
time). If set, the certificates will be issued with a not_before_time of the issuance
time minus the backdate_duration. The not_after_time will be adjusted to preserve the
requested lifetime. The backdate_duration must be less than or equal to 48 hours.</rdfs:comment>
    <rdfs:domain rdf:resource="http://example.org/onto/class/google_privateca_ca_pool"/>
    <rdfs:range rdf:resource="http://www.w3.org/2001/XMLSchema#string"/>
  </owl:DatatypeProperty>
  <owl:DatatypeProperty rdf:about="http://example.org/onto/prop/google_privateca_ca_pool_maximum_lifetime">
    <rdfs:label>maximum_lifetime</rdfs:label>
    <rdfs:comment>The maximum lifetime allowed for issued Certificates. Note that if the issuing CertificateAuthority
expires before a Certificate's requested maximumLifetime, the effective lifetime will be explicitly truncated to match it.</rdfs:comment>
    <rdfs:domain rdf:resource="http://example.org/onto/class/google_privateca_ca_pool"/>
    <rdfs:range rdf:resource="http://www.w3.org/2001/XMLSchema#string"/>
  </owl:DatatypeProperty>
  <owl:DatatypeProperty rdf:about="http://example.org/onto/prop/google_privateca_ca_pool_allow_config_based_issuance">
    <rdfs:label>allow_config_based_issuance</rdfs:label>
    <rdfs:comment>When true, allows callers to create Certificates by specifying a CertificateConfig.</rdfs:comment>
    <rdfs:domain rdf:resource="http://example.org/onto/class/google_privateca_ca_pool"/>
    <rdfs:range rdf:resource="http://www.w3.org/2001/XMLSchema#string"/>
  </owl:DatatypeProperty>
  <owl:DatatypeProperty rdf:about="http://example.org/onto/prop/google_privateca_ca_pool_allow_csr_based_issuance">
    <rdfs:label>allow_csr_based_issuance</rdfs:label>
    <rdfs:comment>When true, allows callers to create Certificates by specifying a CSR.</rdfs:comment>
    <rdfs:domain rdf:resource="http://example.org/onto/class/google_privateca_ca_pool"/>
    <rdfs:range rdf:resource="http://www.w3.org/2001/XMLSchema#string"/>
  </owl:DatatypeProperty>
  <owl:DatatypeProperty rdf:about="http://example.org/onto/prop/google_privateca_ca_pool_signature_algorithm">
    <rdfs:label>signature_algorithm</rdfs:label>
    <rdfs:comment>The algorithm used. Possible values: ["ECDSA_P256", "ECDSA_P384", "EDDSA_25519"]</rdfs:comment>
    <rdfs:domain rdf:resource="http://example.org/onto/class/google_privateca_ca_pool"/>
    <rdfs:range rdf:resource="http://www.w3.org/2001/XMLSchema#string"/>
  </owl:DatatypeProperty>
  <owl:DatatypeProperty rdf:about="http://example.org/onto/prop/google_privateca_ca_pool_max_modulus_size">
    <rdfs:label>max_modulus_size</rdfs:label>
    <rdfs:comment>The maximum allowed RSA modulus size, in bits. If this is not set, or if set to zero, the
service will not enforce an explicit upper bound on RSA modulus sizes.</rdfs:comment>
    <rdfs:domain rdf:resource="http://example.org/onto/class/google_privateca_ca_pool"/>
    <rdfs:range rdf:resource="http://www.w3.org/2001/XMLSchema#string"/>
  </owl:DatatypeProperty>
  <owl:DatatypeProperty rdf:about="http://example.org/onto/prop/google_privateca_ca_pool_min_modulus_size">
    <rdfs:label>min_modulus_size</rdfs:label>
    <rdfs:comment>The minimum allowed RSA modulus size, in bits. If this is not set, or if set to zero, the
service-level min RSA modulus size will continue to apply.</rdfs:comment>
    <rdfs:domain rdf:resource="http://example.org/onto/class/google_privateca_ca_pool"/>
    <rdfs:range rdf:resource="http://www.w3.org/2001/XMLSchema#string"/>
  </owl:DatatypeProperty>
  <owl:DatatypeProperty rdf:about="http://example.org/onto/prop/google_privateca_ca_pool_aia_ocsp_servers">
    <rdfs:label>aia_ocsp_servers</rdfs:label>
    <rdfs:comment>Describes Online Certificate Status Protocol (OCSP) endpoint addresses that appear in the
"Authority Information Access" extension in the certificate.</rdfs:comment>
    <rdfs:domain rdf:resource="http://example.org/onto/class/google_privateca_ca_pool"/>
    <rdfs:range rdf:resource="http://www.w3.org/2001/XMLSchema#string"/>
  </owl:DatatypeProperty>
  <owl:DatatypeProperty rdf:about="http://example.org/onto/prop/google_privateca_ca_pool_critical">
    <rdfs:label>critical</rdfs:label>
    <rdfs:comment>Indicates whether or not this extension is critical (i.e., if the client does not know how to
handle this extension, the client should consider this to be an error).</rdfs:comment>
    <rdfs:domain rdf:resource="http://example.org/onto/class/google_privateca_ca_pool"/>
    <rdfs:range rdf:resource="http://www.w3.org/2001/XMLSchema#string"/>
  </owl:DatatypeProperty>
  <owl:DatatypeProperty rdf:about="http://example.org/onto/prop/google_privateca_ca_pool_value">
    <rdfs:label>value</rdfs:label>
    <rdfs:comment>The value of this X.509 extension. A base64-encoded string.</rdfs:comment>
    <rdfs:domain rdf:resource="http://example.org/onto/class/google_privateca_ca_pool"/>
    <rdfs:range rdf:resource="http://www.w3.org/2001/XMLSchema#string"/>
  </owl:DatatypeProperty>
  <owl:DatatypeProperty rdf:about="http://example.org/onto/prop/google_privateca_ca_pool_object_id_path">
    <rdfs:label>object_id_path</rdfs:label>
    <rdfs:comment>An ObjectId specifies an object identifier (OID). These provide context and describe types in ASN.1 messages.</rdfs:comment>
    <rdfs:domain rdf:resource="http://example.org/onto/class/google_privateca_ca_pool"/>
    <rdfs:range rdf:resource="http://www.w3.org/2001/XMLSchema#string"/>
  </owl:DatatypeProperty>
  <owl:DatatypeProperty rdf:about="http://example.org/onto/prop/google_privateca_ca_pool_is_ca">
    <rdfs:label>is_ca</rdfs:label>
    <rdfs:comment>When true, the "CA" in Basic Constraints extension will be set to true.</rdfs:comment>
    <rdfs:domain rdf:resource="http://example.org/onto/class/google_privateca_ca_pool"/>
    <rdfs:range rdf:resource="http://www.w3.org/2001/XMLSchema#string"/>
  </owl:DatatypeProperty>
  <owl:DatatypeProperty rdf:about="http://example.org/onto/prop/google_privateca_ca_pool_max_issuer_path_length">
    <rdfs:label>max_issuer_path_length</rdfs:label>
    <rdfs:comment>Refers to the "path length constraint" in Basic Constraints extension. For a CA certificate, this value describes the depth of
subordinate CA certificates that are allowed. If this value is less than 0, the request will fail.</rdfs:comment>
    <rdfs:domain rdf:resource="http://example.org/onto/class/google_privateca_ca_pool"/>
    <rdfs:range rdf:resource="http://www.w3.org/2001/XMLSchema#string"/>
  </owl:DatatypeProperty>
  <owl:DatatypeProperty rdf:about="http://example.org/onto/prop/google_privateca_ca_pool_non_ca">
    <rdfs:label>non_ca</rdfs:label>
    <rdfs:comment>When true, the "CA" in Basic Constraints extension will be set to false.
If both 'is_ca' and 'non_ca' are unset, the extension will be omitted from the CA certificate.</rdfs:comment>
    <rdfs:domain rdf:resource="http://example.org/onto/class/google_privateca_ca_pool"/>
    <rdfs:range rdf:resource="http://www.w3.org/2001/XMLSchema#string"/>
  </owl:DatatypeProperty>
  <owl:DatatypeProperty rdf:about="http://example.org/onto/prop/google_privateca_ca_pool_zero_max_issuer_path_length">
    <rdfs:label>zero_max_issuer_path_length</rdfs:label>
    <rdfs:comment>When true, the "path length constraint" in Basic Constraints extension will be set to 0.
if both 'max_issuer_path_length' and 'zero_max_issuer_path_length' are unset,
the max path length will be omitted from the CA certificate.</rdfs:comment>
    <rdfs:domain rdf:resource="http://example.org/onto/class/google_privateca_ca_pool"/>
    <rdfs:range rdf:resource="http://www.w3.org/2001/XMLSchema#string"/>
  </owl:DatatypeProperty>
  <owl:DatatypeProperty rdf:about="http://example.org/onto/prop/google_privateca_ca_pool_cert_sign">
    <rdfs:label>cert_sign</rdfs:label>
    <rdfs:comment>The key may be used to sign certificates.</rdfs:comment>
    <rdfs:domain rdf:resource="http://example.org/onto/class/google_privateca_ca_pool"/>
    <rdfs:range rdf:resource="http://www.w3.org/2001/XMLSchema#string"/>
  </owl:DatatypeProperty>
  <owl:DatatypeProperty rdf:about="http://example.org/onto/prop/google_privateca_ca_pool_content_commitment">
    <rdfs:label>content_commitment</rdfs:label>
    <rdfs:comment>The key may be used for cryptographic commitments. Note that this may also be referred to as "non-repudiation".</rdfs:comment>
    <rdfs:domain rdf:resource="http://example.org/onto/class/google_privateca_ca_pool"/>
    <rdfs:range rdf:resource="http://www.w3.org/2001/XMLSchema#string"/>
  </owl:DatatypeProperty>
  <owl:DatatypeProperty rdf:about="http://example.org/onto/prop/google_privateca_ca_pool_crl_sign">
    <rdfs:label>crl_sign</rdfs:label>
    <rdfs:comment>The key may be used sign certificate revocation lists.</rdfs:comment>
    <rdfs:domain rdf:resource="http://example.org/onto/class/google_privateca_ca_pool"/>
    <rdfs:range rdf:resource="http://www.w3.org/2001/XMLSchema#string"/>
  </owl:DatatypeProperty>
  <owl:DatatypeProperty rdf:about="http://example.org/onto/prop/google_privateca_ca_pool_data_encipherment">
    <rdfs:label>data_encipherment</rdfs:label>
    <rdfs:comment>The key may be used to encipher data.</rdfs:comment>
    <rdfs:domain rdf:resource="http://example.org/onto/class/google_privateca_ca_pool"/>
    <rdfs:range rdf:resource="http://www.w3.org/2001/XMLSchema#string"/>
  </owl:DatatypeProperty>
  <owl:DatatypeProperty rdf:about="http://example.org/onto/prop/google_privateca_ca_pool_decipher_only">
    <rdfs:label>decipher_only</rdfs:label>
    <rdfs:comment>The key may be used to decipher only.</rdfs:comment>
    <rdfs:domain rdf:resource="http://example.org/onto/class/google_privateca_ca_pool"/>
    <rdfs:range rdf:resource="http://www.w3.org/2001/XMLSchema#string"/>
  </owl:DatatypeProperty>
  <owl:DatatypeProperty rdf:about="http://example.org/onto/prop/google_privateca_ca_pool_digital_signature">
    <rdfs:label>digital_signature</rdfs:label>
    <rdfs:comment>The key may be used for digital signatures.</rdfs:comment>
    <rdfs:domain rdf:resource="http://example.org/onto/class/google_privateca_ca_pool"/>
    <rdfs:range rdf:resource="http://www.w3.org/2001/XMLSchema#string"/>
  </owl:DatatypeProperty>
  <owl:DatatypeProperty rdf:about="http://example.org/onto/prop/google_privateca_ca_pool_encipher_only">
    <rdfs:label>encipher_only</rdfs:label>
    <rdfs:comment>The key may be used to encipher only.</rdfs:comment>
    <rdfs:domain rdf:resource="http://example.org/onto/class/google_privateca_ca_pool"/>
    <rdfs:range rdf:resource="http://www.w3.org/2001/XMLSchema#string"/>
  </owl:DatatypeProperty>
  <owl:DatatypeProperty rdf:about="http://example.org/onto/prop/google_privateca_ca_pool_key_agreement">
    <rdfs:label>key_agreement</rdfs:label>
    <rdfs:comment>The key may be used in a key agreement protocol.</rdfs:comment>
    <rdfs:domain rdf:resource="http://example.org/onto/class/google_privateca_ca_pool"/>
    <rdfs:range rdf:resource="http://www.w3.org/2001/XMLSchema#string"/>
  </owl:DatatypeProperty>
  <owl:DatatypeProperty rdf:about="http://example.org/onto/prop/google_privateca_ca_pool_key_encipherment">
    <rdfs:label>key_encipherment</rdfs:label>
    <rdfs:comment>The key may be used to encipher other keys.</rdfs:comment>
    <rdfs:domain rdf:resource="http://example.org/onto/class/google_privateca_ca_pool"/>
    <rdfs:range rdf:resource="http://www.w3.org/2001/XMLSchema#string"/>
  </owl:DatatypeProperty>
  <owl:DatatypeProperty rdf:about="http://example.org/onto/prop/google_privateca_ca_pool_client_auth">
    <rdfs:label>client_auth</rdfs:label>
    <rdfs:comment>Corresponds to OID 1.3.6.1.5.5.7.3.2. Officially described as "TLS WWW client authentication", though regularly used for non-WWW TLS.</rdfs:comment>
    <rdfs:domain rdf:resource="http://example.org/onto/class/google_privateca_ca_pool"/>
    <rdfs:range rdf:resource="http://www.w3.org/2001/XMLSchema#string"/>
  </owl:DatatypeProperty>
  <owl:DatatypeProperty rdf:about="http://example.org/onto/prop/google_privateca_ca_pool_code_signing">
    <rdfs:label>code_signing</rdfs:label>
    <rdfs:comment>Corresponds to OID 1.3.6.1.5.5.7.3.3. Officially described as "Signing of downloadable executable code client authentication".</rdfs:comment>
    <rdfs:domain rdf:resource="http://example.org/onto/class/google_privateca_ca_pool"/>
    <rdfs:range rdf:resource="http://www.w3.org/2001/XMLSchema#string"/>
  </owl:DatatypeProperty>
  <owl:DatatypeProperty rdf:about="http://example.org/onto/prop/google_privateca_ca_pool_email_protection">
    <rdfs:label>email_protection</rdfs:label>
    <rdfs:comment>Corresponds to OID 1.3.6.1.5.5.7.3.4. Officially described as "Email protection".</rdfs:comment>
    <rdfs:domain rdf:resource="http://example.org/onto/class/google_privateca_ca_pool"/>
    <rdfs:range rdf:resource="http://www.w3.org/2001/XMLSchema#string"/>
  </owl:DatatypeProperty>
  <owl:DatatypeProperty rdf:about="http://example.org/onto/prop/google_privateca_ca_pool_ocsp_signing">
    <rdfs:label>ocsp_signing</rdfs:label>
    <rdfs:comment>Corresponds to OID 1.3.6.1.5.5.7.3.9. Officially described as "Signing OCSP responses".</rdfs:comment>
    <rdfs:domain rdf:resource="http://example.org/onto/class/google_privateca_ca_pool"/>
    <rdfs:range rdf:resource="http://www.w3.org/2001/XMLSchema#string"/>
  </owl:DatatypeProperty>
  <owl:DatatypeProperty rdf:about="http://example.org/onto/prop/google_privateca_ca_pool_server_auth">
    <rdfs:label>server_auth</rdfs:label>
    <rdfs:comment>Corresponds to OID 1.3.6.1.5.5.7.3.1. Officially described as "TLS WWW server authentication", though regularly used for non-WWW TLS.</rdfs:comment>
    <rdfs:domain rdf:resource="http://example.org/onto/class/google_privateca_ca_pool"/>
    <rdfs:range rdf:resource="http://www.w3.org/2001/XMLSchema#string"/>
  </owl:DatatypeProperty>
  <owl:DatatypeProperty rdf:about="http://example.org/onto/prop/google_privateca_ca_pool_time_stamping">
    <rdfs:label>time_stamping</rdfs:label>
    <rdfs:comment>Corresponds to OID 1.3.6.1.5.5.7.3.8. Officially described as "Binding the hash of an object to a time".</rdfs:comment>
    <rdfs:domain rdf:resource="http://example.org/onto/class/google_privateca_ca_pool"/>
    <rdfs:range rdf:resource="http://www.w3.org/2001/XMLSchema#string"/>
  </owl:DatatypeProperty>
  <owl:DatatypeProperty rdf:about="http://example.org/onto/prop/google_privateca_ca_pool_object_id_path">
    <rdfs:label>object_id_path</rdfs:label>
    <rdfs:comment>An ObjectId specifies an object identifier (OID). These provide context and describe types in ASN.1 messages.</rdfs:comment>
    <rdfs:domain rdf:resource="http://example.org/onto/class/google_privateca_ca_pool"/>
    <rdfs:range rdf:resource="http://www.w3.org/2001/XMLSchema#string"/>
  </owl:DatatypeProperty>
  <owl:DatatypeProperty rdf:about="http://example.org/onto/prop/google_privateca_ca_pool_critical">
    <rdfs:label>critical</rdfs:label>
    <rdfs:comment>Indicates whether or not the name constraints are marked critical.</rdfs:comment>
    <rdfs:domain rdf:resource="http://example.org/onto/class/google_privateca_ca_pool"/>
    <rdfs:range rdf:resource="http://www.w3.org/2001/XMLSchema#string"/>
  </owl:DatatypeProperty>
  <owl:DatatypeProperty rdf:about="http://example.org/onto/prop/google_privateca_ca_pool_excluded_dns_names">
    <rdfs:label>excluded_dns_names</rdfs:label>
    <rdfs:comment>Contains excluded DNS names. Any DNS name that can be
constructed by simply adding zero or more labels to
the left-hand side of the name satisfies the name constraint.
For example, 'example.com', 'www.example.com', 'www.sub.example.com'
would satisfy 'example.com' while 'example1.com' does not.</rdfs:comment>
    <rdfs:domain rdf:resource="http://example.org/onto/class/google_privateca_ca_pool"/>
    <rdfs:range rdf:resource="http://www.w3.org/2001/XMLSchema#string"/>
  </owl:DatatypeProperty>
  <owl:DatatypeProperty rdf:about="http://example.org/onto/prop/google_privateca_ca_pool_excluded_email_addresses">
    <rdfs:label>excluded_email_addresses</rdfs:label>
    <rdfs:comment>Contains the excluded email addresses. The value can be a particular
email address, a hostname to indicate all email addresses on that host or
a domain with a leading period (e.g. '.example.com') to indicate
all email addresses in that domain.</rdfs:comment>
    <rdfs:domain rdf:resource="http://example.org/onto/class/google_privateca_ca_pool"/>
    <rdfs:range rdf:resource="http://www.w3.org/2001/XMLSchema#string"/>
  </owl:DatatypeProperty>
  <owl:DatatypeProperty rdf:about="http://example.org/onto/prop/google_privateca_ca_pool_excluded_ip_ranges">
    <rdfs:label>excluded_ip_ranges</rdfs:label>
    <rdfs:comment>Contains the excluded IP ranges. For IPv4 addresses, the ranges
are expressed using CIDR notation as specified in RFC 4632.
For IPv6 addresses, the ranges are expressed in similar encoding as IPv4
addresses.</rdfs:comment>
    <rdfs:domain rdf:resource="http://example.org/onto/class/google_privateca_ca_pool"/>
    <rdfs:range rdf:resource="http://www.w3.org/2001/XMLSchema#string"/>
  </owl:DatatypeProperty>
  <owl:DatatypeProperty rdf:about="http://example.org/onto/prop/google_privateca_ca_pool_excluded_uris">
    <rdfs:label>excluded_uris</rdfs:label>
    <rdfs:comment>Contains the excluded URIs that apply to the host part of the name.
The value can be a hostname or a domain with a
leading period (like '.example.com')</rdfs:comment>
    <rdfs:domain rdf:resource="http://example.org/onto/class/google_privateca_ca_pool"/>
    <rdfs:range rdf:resource="http://www.w3.org/2001/XMLSchema#string"/>
  </owl:DatatypeProperty>
  <owl:DatatypeProperty rdf:about="http://example.org/onto/prop/google_privateca_ca_pool_permitted_dns_names">
    <rdfs:label>permitted_dns_names</rdfs:label>
    <rdfs:comment>Contains permitted DNS names. Any DNS name that can be
constructed by simply adding zero or more labels to
the left-hand side of the name satisfies the name constraint.
For example, 'example.com', 'www.example.com', 'www.sub.example.com'
would satisfy 'example.com' while 'example1.com' does not.</rdfs:comment>
    <rdfs:domain rdf:resource="http://example.org/onto/class/google_privateca_ca_pool"/>
    <rdfs:range rdf:resource="http://www.w3.org/2001/XMLSchema#string"/>
  </owl:DatatypeProperty>
  <owl:DatatypeProperty rdf:about="http://example.org/onto/prop/google_privateca_ca_pool_permitted_email_addresses">
    <rdfs:label>permitted_email_addresses</rdfs:label>
    <rdfs:comment>Contains the permitted email addresses. The value can be a particular
email address, a hostname to indicate all email addresses on that host or
a domain with a leading period (e.g. '.example.com') to indicate
all email addresses in that domain.</rdfs:comment>
    <rdfs:domain rdf:resource="http://example.org/onto/class/google_privateca_ca_pool"/>
    <rdfs:range rdf:resource="http://www.w3.org/2001/XMLSchema#string"/>
  </owl:DatatypeProperty>
  <owl:DatatypeProperty rdf:about="http://example.org/onto/prop/google_privateca_ca_pool_permitted_ip_ranges">
    <rdfs:label>permitted_ip_ranges</rdfs:label>
    <rdfs:comment>Contains the permitted IP ranges. For IPv4 addresses, the ranges
are expressed using CIDR notation as specified in RFC 4632.
For IPv6 addresses, the ranges are expressed in similar encoding as IPv4
addresses.</rdfs:comment>
    <rdfs:domain rdf:resource="http://example.org/onto/class/google_privateca_ca_pool"/>
    <rdfs:range rdf:resource="http://www.w3.org/2001/XMLSchema#string"/>
  </owl:DatatypeProperty>
  <owl:DatatypeProperty rdf:about="http://example.org/onto/prop/google_privateca_ca_pool_permitted_uris">
    <rdfs:label>permitted_uris</rdfs:label>
    <rdfs:comment>Contains the permitted URIs that apply to the host part of the name.
The value can be a hostname or a domain with a
leading period (like '.example.com')</rdfs:comment>
    <rdfs:domain rdf:resource="http://example.org/onto/class/google_privateca_ca_pool"/>
    <rdfs:range rdf:resource="http://www.w3.org/2001/XMLSchema#string"/>
  </owl:DatatypeProperty>
  <owl:DatatypeProperty rdf:about="http://example.org/onto/prop/google_privateca_ca_pool_object_id_path">
    <rdfs:label>object_id_path</rdfs:label>
    <rdfs:comment>An ObjectId specifies an object identifier (OID). These provide context and describe types in ASN.1 messages.</rdfs:comment>
    <rdfs:domain rdf:resource="http://example.org/onto/class/google_privateca_ca_pool"/>
    <rdfs:range rdf:resource="http://www.w3.org/2001/XMLSchema#string"/>
  </owl:DatatypeProperty>
  <owl:DatatypeProperty rdf:about="http://example.org/onto/prop/google_privateca_ca_pool_allow_subject_alt_names_passthrough">
    <rdfs:label>allow_subject_alt_names_passthrough</rdfs:label>
    <rdfs:comment>If this is set, the SubjectAltNames extension may be copied from a certificate request into the signed certificate.
Otherwise, the requested SubjectAltNames will be discarded.</rdfs:comment>
    <rdfs:domain rdf:resource="http://example.org/onto/class/google_privateca_ca_pool"/>
    <rdfs:range rdf:resource="http://www.w3.org/2001/XMLSchema#string"/>
  </owl:DatatypeProperty>
  <owl:DatatypeProperty rdf:about="http://example.org/onto/prop/google_privateca_ca_pool_allow_subject_passthrough">
    <rdfs:label>allow_subject_passthrough</rdfs:label>
    <rdfs:comment>If this is set, the Subject field may be copied from a certificate request into the signed certificate.
Otherwise, the requested Subject will be discarded.</rdfs:comment>
    <rdfs:domain rdf:resource="http://example.org/onto/class/google_privateca_ca_pool"/>
    <rdfs:range rdf:resource="http://www.w3.org/2001/XMLSchema#string"/>
  </owl:DatatypeProperty>
  <owl:DatatypeProperty rdf:about="http://example.org/onto/prop/google_privateca_ca_pool_description">
    <rdfs:label>description</rdfs:label>
    <rdfs:comment>Description of the expression. This is a longer text which describes the expression, e.g. when hovered over it in a UI.</rdfs:comment>
    <rdfs:domain rdf:resource="http://example.org/onto/class/google_privateca_ca_pool"/>
    <rdfs:range rdf:resource="http://www.w3.org/2001/XMLSchema#string"/>
  </owl:DatatypeProperty>
  <owl:DatatypeProperty rdf:about="http://example.org/onto/prop/google_privateca_ca_pool_expression">
    <rdfs:label>expression</rdfs:label>
    <rdfs:comment>Textual representation of an expression in Common Expression Language syntax.</rdfs:comment>
    <rdfs:domain rdf:resource="http://example.org/onto/class/google_privateca_ca_pool"/>
    <rdfs:range rdf:resource="http://www.w3.org/2001/XMLSchema#string"/>
  </owl:DatatypeProperty>
  <owl:DatatypeProperty rdf:about="http://example.org/onto/prop/google_privateca_ca_pool_location">
    <rdfs:label>location</rdfs:label>
    <rdfs:comment>String indicating the location of the expression for error reporting, e.g. a file name and a position in the file.</rdfs:comment>
    <rdfs:domain rdf:resource="http://example.org/onto/class/google_privateca_ca_pool"/>
    <rdfs:range rdf:resource="http://www.w3.org/2001/XMLSchema#string"/>
  </owl:DatatypeProperty>
  <owl:DatatypeProperty rdf:about="http://example.org/onto/prop/google_privateca_ca_pool_title">
    <rdfs:label>title</rdfs:label>
    <rdfs:comment>Title for the expression, i.e. a short string describing its purpose. This can be used e.g. in UIs which allow to enter the expression.</rdfs:comment>
    <rdfs:domain rdf:resource="http://example.org/onto/class/google_privateca_ca_pool"/>
    <rdfs:range rdf:resource="http://www.w3.org/2001/XMLSchema#string"/>
  </owl:DatatypeProperty>
  <owl:DatatypeProperty rdf:about="http://example.org/onto/prop/google_privateca_ca_pool_encoding_format">
    <rdfs:label>encoding_format</rdfs:label>
    <rdfs:comment>Specifies the encoding format of each CertificateAuthority's CA
certificate and CRLs. If this is omitted, CA certificates and CRLs
will be published in PEM. Possible values: ["PEM", "DER"]</rdfs:comment>
    <rdfs:domain rdf:resource="http://example.org/onto/class/google_privateca_ca_pool"/>
    <rdfs:range rdf:resource="http://www.w3.org/2001/XMLSchema#string"/>
  </owl:DatatypeProperty>
  <owl:DatatypeProperty rdf:about="http://example.org/onto/prop/google_privateca_ca_pool_publish_ca_cert">
    <rdfs:label>publish_ca_cert</rdfs:label>
    <rdfs:comment>When true, publishes each CertificateAuthority's CA certificate and includes its URL in the "Authority Information Access"
X.509 extension in all issued Certificates. If this is false, the CA certificate will not be published and the corresponding
X.509 extension will not be written in issued certificates.</rdfs:comment>
    <rdfs:domain rdf:resource="http://example.org/onto/class/google_privateca_ca_pool"/>
    <rdfs:range rdf:resource="http://www.w3.org/2001/XMLSchema#string"/>
  </owl:DatatypeProperty>
  <owl:DatatypeProperty rdf:about="http://example.org/onto/prop/google_privateca_ca_pool_publish_crl">
    <rdfs:label>publish_crl</rdfs:label>
    <rdfs:comment>When true, publishes each CertificateAuthority's CRL and includes its URL in the "CRL Distribution Points" X.509 extension
in all issued Certificates. If this is false, CRLs will not be published and the corresponding X.509 extension will not
be written in issued certificates. CRLs will expire 7 days from their creation. However, we will rebuild daily. CRLs are
also rebuilt shortly after a certificate is revoked.</rdfs:comment>
    <rdfs:domain rdf:resource="http://example.org/onto/class/google_privateca_ca_pool"/>
    <rdfs:range rdf:resource="http://www.w3.org/2001/XMLSchema#string"/>
  </owl:DatatypeProperty>
  <owl:DatatypeProperty rdf:about="http://example.org/onto/prop/google_privateca_ca_pool_create">
    <rdfs:label>create</rdfs:label>
    <rdfs:domain rdf:resource="http://example.org/onto/class/google_privateca_ca_pool"/>
    <rdfs:range rdf:resource="http://www.w3.org/2001/XMLSchema#string"/>
  </owl:DatatypeProperty>
  <owl:DatatypeProperty rdf:about="http://example.org/onto/prop/google_privateca_ca_pool_delete">
    <rdfs:label>delete</rdfs:label>
    <rdfs:domain rdf:resource="http://example.org/onto/class/google_privateca_ca_pool"/>
    <rdfs:range rdf:resource="http://www.w3.org/2001/XMLSchema#string"/>
  </owl:DatatypeProperty>
  <owl:DatatypeProperty rdf:about="http://example.org/onto/prop/google_privateca_ca_pool_update">
    <rdfs:label>update</rdfs:label>
    <rdfs:domain rdf:resource="http://example.org/onto/class/google_privateca_ca_pool"/>
    <rdfs:range rdf:resource="http://www.w3.org/2001/XMLSchema#string"/>
  </owl:DatatypeProperty>
</rdf:RDF>
