<?xml version="1.0" encoding="UTF-8"?>
<rdf:RDF
  xmlns:rdf="http://www.w3.org/1999/02/22-rdf-syntax-ns#"
  xmlns:rdfs="http://www.w3.org/2000/01/rdf-schema#"
  xmlns:owl="http://www.w3.org/2002/07/owl#"
  xmlns:xsd="http://www.w3.org/2001/XMLSchema#"
  xml:base="http://example.org/onto/">
  <owl:Class rdf:about="http://example.org/onto/class/google_compute_region_security_policy">
    <rdfs:label>google_compute_region_security_policy</rdfs:label>
    <rdfs:comment>#
#     ***     AUTO GENERATED CODE    ***    Type: MMv1     ***
#
# ----------------------------------------------------------------------------
#
#     This code is generated by Magic Modules using the following:
#
#     Configuration: https:#github.com/GoogleCloudPlatform/magic-modules/tree/main/mmv1/products/compute/RegionSecurityPolicy.yaml
#     Template:      https:#github.com/GoogleCloudPlatform/magic-modules/tree/main/mmv1/templates/terraform/resource.html.markdown.tmpl
#
#     DO NOT EDIT this file directly. Any changes made to this file will be
#     overwritten during the next generation cycle.
#
# ----------------------------------------------------------------------------
subcategory: "Compute Engine"
description: |-
  Represents a Region Cloud Armor Security Policy resource.
---</rdfs:comment>
  </owl:Class>
  <owl:DatatypeProperty rdf:about="http://example.org/onto/prop/google_compute_region_security_policy_description">
    <rdfs:label>description</rdfs:label>
    <rdfs:comment>An optional description of this resource. Provide this property when you create the resource.</rdfs:comment>
    <rdfs:domain rdf:resource="http://example.org/onto/class/google_compute_region_security_policy"/>
    <rdfs:range rdf:resource="http://www.w3.org/2001/XMLSchema#string"/>
  </owl:DatatypeProperty>
  <owl:DatatypeProperty rdf:about="http://example.org/onto/prop/google_compute_region_security_policy_fingerprint">
    <rdfs:label>fingerprint</rdfs:label>
    <rdfs:comment>Fingerprint of this resource. This field is used internally during
updates of this resource.</rdfs:comment>
    <rdfs:domain rdf:resource="http://example.org/onto/class/google_compute_region_security_policy"/>
    <rdfs:range rdf:resource="http://www.w3.org/2001/XMLSchema#string"/>
  </owl:DatatypeProperty>
  <owl:DatatypeProperty rdf:about="http://example.org/onto/prop/google_compute_region_security_policy_id">
    <rdfs:label>id</rdfs:label>
    <rdfs:domain rdf:resource="http://example.org/onto/class/google_compute_region_security_policy"/>
    <rdfs:range rdf:resource="http://www.w3.org/2001/XMLSchema#string"/>
  </owl:DatatypeProperty>
  <owl:DatatypeProperty rdf:about="http://example.org/onto/prop/google_compute_region_security_policy_name">
    <rdfs:label>name</rdfs:label>
    <rdfs:comment>Name of the resource. Provided by the client when the resource is created. The name must be 1-63 characters long, and comply with RFC1035.
Specifically, the name must be 1-63 characters long and match the regular expression [a-z]([-a-z0-9]*[a-z0-9])? which means the first character must be a lowercase letter, and all following characters must be a dash, lowercase letter, or digit, except the last character, which cannot be a dash.</rdfs:comment>
    <rdfs:domain rdf:resource="http://example.org/onto/class/google_compute_region_security_policy"/>
    <rdfs:range rdf:resource="http://www.w3.org/2001/XMLSchema#string"/>
  </owl:DatatypeProperty>
  <owl:DatatypeProperty rdf:about="http://example.org/onto/prop/google_compute_region_security_policy_policy_id">
    <rdfs:label>policy_id</rdfs:label>
    <rdfs:comment>The unique identifier for the resource. This identifier is defined by the server.</rdfs:comment>
    <rdfs:domain rdf:resource="http://example.org/onto/class/google_compute_region_security_policy"/>
    <rdfs:range rdf:resource="http://www.w3.org/2001/XMLSchema#string"/>
  </owl:DatatypeProperty>
  <owl:DatatypeProperty rdf:about="http://example.org/onto/prop/google_compute_region_security_policy_project">
    <rdfs:label>project</rdfs:label>
    <rdfs:domain rdf:resource="http://example.org/onto/class/google_compute_region_security_policy"/>
    <rdfs:range rdf:resource="http://www.w3.org/2001/XMLSchema#string"/>
  </owl:DatatypeProperty>
  <owl:DatatypeProperty rdf:about="http://example.org/onto/prop/google_compute_region_security_policy_region">
    <rdfs:label>region</rdfs:label>
    <rdfs:comment>The Region in which the created Region Security Policy should reside.
If it is not provided, the provider region is used.</rdfs:comment>
    <rdfs:domain rdf:resource="http://example.org/onto/class/google_compute_region_security_policy"/>
    <rdfs:range rdf:resource="http://www.w3.org/2001/XMLSchema#string"/>
  </owl:DatatypeProperty>
  <owl:DatatypeProperty rdf:about="http://example.org/onto/prop/google_compute_region_security_policy_self_link">
    <rdfs:label>self_link</rdfs:label>
    <rdfs:comment>Server-defined URL for the resource.</rdfs:comment>
    <rdfs:domain rdf:resource="http://example.org/onto/class/google_compute_region_security_policy"/>
    <rdfs:range rdf:resource="http://www.w3.org/2001/XMLSchema#string"/>
  </owl:DatatypeProperty>
  <owl:DatatypeProperty rdf:about="http://example.org/onto/prop/google_compute_region_security_policy_self_link_with_policy_id">
    <rdfs:label>self_link_with_policy_id</rdfs:label>
    <rdfs:comment>Server-defined URL for this resource with the resource id.</rdfs:comment>
    <rdfs:domain rdf:resource="http://example.org/onto/class/google_compute_region_security_policy"/>
    <rdfs:range rdf:resource="http://www.w3.org/2001/XMLSchema#string"/>
  </owl:DatatypeProperty>
  <owl:DatatypeProperty rdf:about="http://example.org/onto/prop/google_compute_region_security_policy_type">
    <rdfs:label>type</rdfs:label>
    <rdfs:comment>The type indicates the intended use of the security policy.
- CLOUD_ARMOR: Cloud Armor backend security policies can be configured to filter incoming HTTP requests targeting backend services. They filter requests before they hit the origin servers.
- CLOUD_ARMOR_EDGE: Cloud Armor edge security policies can be configured to filter incoming HTTP requests targeting backend services (including Cloud CDN-enabled) as well as backend buckets (Cloud Storage). They filter requests before the request is served from Google's cache.
- CLOUD_ARMOR_NETWORK: Cloud Armor network policies can be configured to filter packets targeting network load balancing resources such as backend services, target pools, target instances, and instances with external IPs. They filter requests before the request is served from the application.
This field can be set only at resource creation time. Possible values: ["CLOUD_ARMOR", "CLOUD_ARMOR_EDGE", "CLOUD_ARMOR_NETWORK"]</rdfs:comment>
    <rdfs:domain rdf:resource="http://example.org/onto/class/google_compute_region_security_policy"/>
    <rdfs:range rdf:resource="http://www.w3.org/2001/XMLSchema#string"/>
  </owl:DatatypeProperty>
  <owl:DatatypeProperty rdf:about="http://example.org/onto/prop/google_compute_region_security_policy_json_parsing">
    <rdfs:label>json_parsing</rdfs:label>
    <rdfs:comment>JSON body parsing. Supported values include: "DISABLED", "STANDARD", "STANDARD_WITH_GRAPHQL". Possible values: ["DISABLED", "STANDARD", "STANDARD_WITH_GRAPHQL"]</rdfs:comment>
    <rdfs:domain rdf:resource="http://example.org/onto/class/google_compute_region_security_policy"/>
    <rdfs:range rdf:resource="http://www.w3.org/2001/XMLSchema#string"/>
  </owl:DatatypeProperty>
  <owl:DatatypeProperty rdf:about="http://example.org/onto/prop/google_compute_region_security_policy_log_level">
    <rdfs:label>log_level</rdfs:label>
    <rdfs:comment>Logging level. Supported values include: "NORMAL", "VERBOSE". Possible values: ["NORMAL", "VERBOSE"]</rdfs:comment>
    <rdfs:domain rdf:resource="http://example.org/onto/class/google_compute_region_security_policy"/>
    <rdfs:range rdf:resource="http://www.w3.org/2001/XMLSchema#string"/>
  </owl:DatatypeProperty>
  <owl:DatatypeProperty rdf:about="http://example.org/onto/prop/google_compute_region_security_policy_user_ip_request_headers">
    <rdfs:label>user_ip_request_headers</rdfs:label>
    <rdfs:comment>An optional list of case-insensitive request header names to use for resolving the callers client IP address.</rdfs:comment>
    <rdfs:domain rdf:resource="http://example.org/onto/class/google_compute_region_security_policy"/>
    <rdfs:range rdf:resource="http://www.w3.org/2001/XMLSchema#string"/>
  </owl:DatatypeProperty>
  <owl:DatatypeProperty rdf:about="http://example.org/onto/prop/google_compute_region_security_policy_content_types">
    <rdfs:label>content_types</rdfs:label>
    <rdfs:comment>A list of custom Content-Type header values to apply the JSON parsing.</rdfs:comment>
    <rdfs:domain rdf:resource="http://example.org/onto/class/google_compute_region_security_policy"/>
    <rdfs:range rdf:resource="http://www.w3.org/2001/XMLSchema#string"/>
  </owl:DatatypeProperty>
  <owl:DatatypeProperty rdf:about="http://example.org/onto/prop/google_compute_region_security_policy_ddos_protection">
    <rdfs:label>ddos_protection</rdfs:label>
    <rdfs:comment>Google Cloud Armor offers the following options to help protect systems against DDoS attacks:
- STANDARD: basic always-on protection for network load balancers, protocol forwarding, or VMs with public IP addresses.
- ADVANCED: additional protections for Managed Protection Plus subscribers who use network load balancers, protocol forwarding, or VMs with public IP addresses.
- ADVANCED_PREVIEW: flag to enable the security policy in preview mode. Possible values: ["ADVANCED", "ADVANCED_PREVIEW", "STANDARD"]</rdfs:comment>
    <rdfs:domain rdf:resource="http://example.org/onto/class/google_compute_region_security_policy"/>
    <rdfs:range rdf:resource="http://www.w3.org/2001/XMLSchema#string"/>
  </owl:DatatypeProperty>
  <owl:DatatypeProperty rdf:about="http://example.org/onto/prop/google_compute_region_security_policy_action">
    <rdfs:label>action</rdfs:label>
    <rdfs:comment>The Action to perform when the rule is matched. The following are the valid actions:

* allow: allow access to target.

* deny(STATUS): deny access to target, returns the HTTP response code specified. Valid values for STATUS are 403, 404, and 502.

* rate_based_ban: limit client traffic to the configured threshold and ban the client if the traffic exceeds the threshold. Configure parameters for this action in RateLimitOptions. Requires rateLimitOptions to be set.

* redirect: redirect to a different target. This can either be an internal reCAPTCHA redirect, or an external URL-based redirect via a 302 response. Parameters for this action can be configured via redirectOptions. This action is only supported in Global Security Policies of type CLOUD_ARMOR.

* throttle: limit client traffic to the configured threshold. Configure parameters for this action in rateLimitOptions. Requires rateLimitOptions to be set for this.</rdfs:comment>
    <rdfs:domain rdf:resource="http://example.org/onto/class/google_compute_region_security_policy"/>
    <rdfs:range rdf:resource="http://www.w3.org/2001/XMLSchema#string"/>
  </owl:DatatypeProperty>
  <owl:DatatypeProperty rdf:about="http://example.org/onto/prop/google_compute_region_security_policy_description">
    <rdfs:label>description</rdfs:label>
    <rdfs:comment>An optional description of this resource. Provide this property when you create the resource.</rdfs:comment>
    <rdfs:domain rdf:resource="http://example.org/onto/class/google_compute_region_security_policy"/>
    <rdfs:range rdf:resource="http://www.w3.org/2001/XMLSchema#string"/>
  </owl:DatatypeProperty>
  <owl:DatatypeProperty rdf:about="http://example.org/onto/prop/google_compute_region_security_policy_preview">
    <rdfs:label>preview</rdfs:label>
    <rdfs:comment>If set to true, the specified action is not enforced.</rdfs:comment>
    <rdfs:domain rdf:resource="http://example.org/onto/class/google_compute_region_security_policy"/>
    <rdfs:range rdf:resource="http://www.w3.org/2001/XMLSchema#string"/>
  </owl:DatatypeProperty>
  <owl:DatatypeProperty rdf:about="http://example.org/onto/prop/google_compute_region_security_policy_priority">
    <rdfs:label>priority</rdfs:label>
    <rdfs:comment>An integer indicating the priority of a rule in the list.
The priority must be a positive value between 0 and 2147483647.
Rules are evaluated from highest to lowest priority where 0 is the highest priority and 2147483647 is the lowest priority.</rdfs:comment>
    <rdfs:domain rdf:resource="http://example.org/onto/class/google_compute_region_security_policy"/>
    <rdfs:range rdf:resource="http://www.w3.org/2001/XMLSchema#string"/>
  </owl:DatatypeProperty>
  <owl:DatatypeProperty rdf:about="http://example.org/onto/prop/google_compute_region_security_policy_versioned_expr">
    <rdfs:label>versioned_expr</rdfs:label>
    <rdfs:comment>Preconfigured versioned expression. If this field is specified, config must also be specified.
Available preconfigured expressions along with their requirements are: SRC_IPS_V1 - must specify the corresponding srcIpRange field in config. Possible values: ["SRC_IPS_V1"]</rdfs:comment>
    <rdfs:domain rdf:resource="http://example.org/onto/class/google_compute_region_security_policy"/>
    <rdfs:range rdf:resource="http://www.w3.org/2001/XMLSchema#string"/>
  </owl:DatatypeProperty>
  <owl:DatatypeProperty rdf:about="http://example.org/onto/prop/google_compute_region_security_policy_src_ip_ranges">
    <rdfs:label>src_ip_ranges</rdfs:label>
    <rdfs:comment>CIDR IP address range. Maximum number of srcIpRanges allowed is 10.</rdfs:comment>
    <rdfs:domain rdf:resource="http://example.org/onto/class/google_compute_region_security_policy"/>
    <rdfs:range rdf:resource="http://www.w3.org/2001/XMLSchema#string"/>
  </owl:DatatypeProperty>
  <owl:DatatypeProperty rdf:about="http://example.org/onto/prop/google_compute_region_security_policy_expression">
    <rdfs:label>expression</rdfs:label>
    <rdfs:comment>Textual representation of an expression in Common Expression Language syntax. The application context of the containing message determines which well-known feature set of CEL is supported.</rdfs:comment>
    <rdfs:domain rdf:resource="http://example.org/onto/class/google_compute_region_security_policy"/>
    <rdfs:range rdf:resource="http://www.w3.org/2001/XMLSchema#string"/>
  </owl:DatatypeProperty>
  <owl:DatatypeProperty rdf:about="http://example.org/onto/prop/google_compute_region_security_policy_dest_ip_ranges">
    <rdfs:label>dest_ip_ranges</rdfs:label>
    <rdfs:comment>Destination IPv4/IPv6 addresses or CIDR prefixes, in standard text format.</rdfs:comment>
    <rdfs:domain rdf:resource="http://example.org/onto/class/google_compute_region_security_policy"/>
    <rdfs:range rdf:resource="http://www.w3.org/2001/XMLSchema#string"/>
  </owl:DatatypeProperty>
  <owl:DatatypeProperty rdf:about="http://example.org/onto/prop/google_compute_region_security_policy_dest_ports">
    <rdfs:label>dest_ports</rdfs:label>
    <rdfs:comment>Destination port numbers for TCP/UDP/SCTP. Each element can be a 16-bit unsigned decimal number (e.g. "80") or range (e.g. "0-1023").</rdfs:comment>
    <rdfs:domain rdf:resource="http://example.org/onto/class/google_compute_region_security_policy"/>
    <rdfs:range rdf:resource="http://www.w3.org/2001/XMLSchema#string"/>
  </owl:DatatypeProperty>
  <owl:DatatypeProperty rdf:about="http://example.org/onto/prop/google_compute_region_security_policy_ip_protocols">
    <rdfs:label>ip_protocols</rdfs:label>
    <rdfs:comment>IPv4 protocol / IPv6 next header (after extension headers). Each element can be an 8-bit unsigned decimal number (e.g. "6"), range (e.g. "253-254"), or one of the following protocol names: "tcp", "udp", "icmp", "esp", "ah", "ipip", or "sctp".</rdfs:comment>
    <rdfs:domain rdf:resource="http://example.org/onto/class/google_compute_region_security_policy"/>
    <rdfs:range rdf:resource="http://www.w3.org/2001/XMLSchema#string"/>
  </owl:DatatypeProperty>
  <owl:DatatypeProperty rdf:about="http://example.org/onto/prop/google_compute_region_security_policy_src_asns">
    <rdfs:label>src_asns</rdfs:label>
    <rdfs:comment>BGP Autonomous System Number associated with the source IP address.</rdfs:comment>
    <rdfs:domain rdf:resource="http://example.org/onto/class/google_compute_region_security_policy"/>
    <rdfs:range rdf:resource="http://www.w3.org/2001/XMLSchema#string"/>
  </owl:DatatypeProperty>
  <owl:DatatypeProperty rdf:about="http://example.org/onto/prop/google_compute_region_security_policy_src_ip_ranges">
    <rdfs:label>src_ip_ranges</rdfs:label>
    <rdfs:comment>Source IPv4/IPv6 addresses or CIDR prefixes, in standard text format.</rdfs:comment>
    <rdfs:domain rdf:resource="http://example.org/onto/class/google_compute_region_security_policy"/>
    <rdfs:range rdf:resource="http://www.w3.org/2001/XMLSchema#string"/>
  </owl:DatatypeProperty>
  <owl:DatatypeProperty rdf:about="http://example.org/onto/prop/google_compute_region_security_policy_src_ports">
    <rdfs:label>src_ports</rdfs:label>
    <rdfs:comment>Source port numbers for TCP/UDP/SCTP. Each element can be a 16-bit unsigned decimal number (e.g. "80") or range (e.g. "0-1023").</rdfs:comment>
    <rdfs:domain rdf:resource="http://example.org/onto/class/google_compute_region_security_policy"/>
    <rdfs:range rdf:resource="http://www.w3.org/2001/XMLSchema#string"/>
  </owl:DatatypeProperty>
  <owl:DatatypeProperty rdf:about="http://example.org/onto/prop/google_compute_region_security_policy_src_region_codes">
    <rdfs:label>src_region_codes</rdfs:label>
    <rdfs:comment>Two-letter ISO 3166-1 alpha-2 country code associated with the source IP address.</rdfs:comment>
    <rdfs:domain rdf:resource="http://example.org/onto/class/google_compute_region_security_policy"/>
    <rdfs:range rdf:resource="http://www.w3.org/2001/XMLSchema#string"/>
  </owl:DatatypeProperty>
  <owl:DatatypeProperty rdf:about="http://example.org/onto/prop/google_compute_region_security_policy_name">
    <rdfs:label>name</rdfs:label>
    <rdfs:comment>Name of the user-defined field, as given in the definition.</rdfs:comment>
    <rdfs:domain rdf:resource="http://example.org/onto/class/google_compute_region_security_policy"/>
    <rdfs:range rdf:resource="http://www.w3.org/2001/XMLSchema#string"/>
  </owl:DatatypeProperty>
  <owl:DatatypeProperty rdf:about="http://example.org/onto/prop/google_compute_region_security_policy_values">
    <rdfs:label>values</rdfs:label>
    <rdfs:comment>Matching values of the field. Each element can be a 32-bit unsigned decimal or hexadecimal (starting with "0x") number (e.g. "64") or range (e.g. "0x400-0x7ff").</rdfs:comment>
    <rdfs:domain rdf:resource="http://example.org/onto/class/google_compute_region_security_policy"/>
    <rdfs:range rdf:resource="http://www.w3.org/2001/XMLSchema#string"/>
  </owl:DatatypeProperty>
  <owl:DatatypeProperty rdf:about="http://example.org/onto/prop/google_compute_region_security_policy_target_rule_ids">
    <rdfs:label>target_rule_ids</rdfs:label>
    <rdfs:comment>A list of target rule IDs under the WAF rule set to apply the preconfigured WAF exclusion.
If omitted, it refers to all the rule IDs under the WAF rule set.</rdfs:comment>
    <rdfs:domain rdf:resource="http://example.org/onto/class/google_compute_region_security_policy"/>
    <rdfs:range rdf:resource="http://www.w3.org/2001/XMLSchema#string"/>
  </owl:DatatypeProperty>
  <owl:DatatypeProperty rdf:about="http://example.org/onto/prop/google_compute_region_security_policy_target_rule_set">
    <rdfs:label>target_rule_set</rdfs:label>
    <rdfs:comment>Target WAF rule set to apply the preconfigured WAF exclusion.</rdfs:comment>
    <rdfs:domain rdf:resource="http://example.org/onto/class/google_compute_region_security_policy"/>
    <rdfs:range rdf:resource="http://www.w3.org/2001/XMLSchema#string"/>
  </owl:DatatypeProperty>
  <owl:DatatypeProperty rdf:about="http://example.org/onto/prop/google_compute_region_security_policy_operator">
    <rdfs:label>operator</rdfs:label>
    <rdfs:comment>You can specify an exact match or a partial match by using a field operator and a field value.
Available options:
EQUALS: The operator matches if the field value equals the specified value.
STARTS_WITH: The operator matches if the field value starts with the specified value.
ENDS_WITH: The operator matches if the field value ends with the specified value.
CONTAINS: The operator matches if the field value contains the specified value.
EQUALS_ANY: The operator matches if the field value is any value. Possible values: ["CONTAINS", "ENDS_WITH", "EQUALS", "EQUALS_ANY", "STARTS_WITH"]</rdfs:comment>
    <rdfs:domain rdf:resource="http://example.org/onto/class/google_compute_region_security_policy"/>
    <rdfs:range rdf:resource="http://www.w3.org/2001/XMLSchema#string"/>
  </owl:DatatypeProperty>
  <owl:DatatypeProperty rdf:about="http://example.org/onto/prop/google_compute_region_security_policy_value">
    <rdfs:label>value</rdfs:label>
    <rdfs:comment>A request field matching the specified value will be excluded from inspection during preconfigured WAF evaluation.
The field value must be given if the field operator is not EQUALS_ANY, and cannot be given if the field operator is EQUALS_ANY.</rdfs:comment>
    <rdfs:domain rdf:resource="http://example.org/onto/class/google_compute_region_security_policy"/>
    <rdfs:range rdf:resource="http://www.w3.org/2001/XMLSchema#string"/>
  </owl:DatatypeProperty>
  <owl:DatatypeProperty rdf:about="http://example.org/onto/prop/google_compute_region_security_policy_operator">
    <rdfs:label>operator</rdfs:label>
    <rdfs:comment>You can specify an exact match or a partial match by using a field operator and a field value.
Available options:
EQUALS: The operator matches if the field value equals the specified value.
STARTS_WITH: The operator matches if the field value starts with the specified value.
ENDS_WITH: The operator matches if the field value ends with the specified value.
CONTAINS: The operator matches if the field value contains the specified value.
EQUALS_ANY: The operator matches if the field value is any value. Possible values: ["CONTAINS", "ENDS_WITH", "EQUALS", "EQUALS_ANY", "STARTS_WITH"]</rdfs:comment>
    <rdfs:domain rdf:resource="http://example.org/onto/class/google_compute_region_security_policy"/>
    <rdfs:range rdf:resource="http://www.w3.org/2001/XMLSchema#string"/>
  </owl:DatatypeProperty>
  <owl:DatatypeProperty rdf:about="http://example.org/onto/prop/google_compute_region_security_policy_value">
    <rdfs:label>value</rdfs:label>
    <rdfs:comment>A request field matching the specified value will be excluded from inspection during preconfigured WAF evaluation.
The field value must be given if the field operator is not EQUALS_ANY, and cannot be given if the field operator is EQUALS_ANY.</rdfs:comment>
    <rdfs:domain rdf:resource="http://example.org/onto/class/google_compute_region_security_policy"/>
    <rdfs:range rdf:resource="http://www.w3.org/2001/XMLSchema#string"/>
  </owl:DatatypeProperty>
  <owl:DatatypeProperty rdf:about="http://example.org/onto/prop/google_compute_region_security_policy_operator">
    <rdfs:label>operator</rdfs:label>
    <rdfs:comment>You can specify an exact match or a partial match by using a field operator and a field value.
Available options:
EQUALS: The operator matches if the field value equals the specified value.
STARTS_WITH: The operator matches if the field value starts with the specified value.
ENDS_WITH: The operator matches if the field value ends with the specified value.
CONTAINS: The operator matches if the field value contains the specified value.
EQUALS_ANY: The operator matches if the field value is any value. Possible values: ["CONTAINS", "ENDS_WITH", "EQUALS", "EQUALS_ANY", "STARTS_WITH"]</rdfs:comment>
    <rdfs:domain rdf:resource="http://example.org/onto/class/google_compute_region_security_policy"/>
    <rdfs:range rdf:resource="http://www.w3.org/2001/XMLSchema#string"/>
  </owl:DatatypeProperty>
  <owl:DatatypeProperty rdf:about="http://example.org/onto/prop/google_compute_region_security_policy_value">
    <rdfs:label>value</rdfs:label>
    <rdfs:comment>A request field matching the specified value will be excluded from inspection during preconfigured WAF evaluation.
The field value must be given if the field operator is not EQUALS_ANY, and cannot be given if the field operator is EQUALS_ANY.</rdfs:comment>
    <rdfs:domain rdf:resource="http://example.org/onto/class/google_compute_region_security_policy"/>
    <rdfs:range rdf:resource="http://www.w3.org/2001/XMLSchema#string"/>
  </owl:DatatypeProperty>
  <owl:DatatypeProperty rdf:about="http://example.org/onto/prop/google_compute_region_security_policy_operator">
    <rdfs:label>operator</rdfs:label>
    <rdfs:comment>You can specify an exact match or a partial match by using a field operator and a field value.
Available options:
EQUALS: The operator matches if the field value equals the specified value.
STARTS_WITH: The operator matches if the field value starts with the specified value.
ENDS_WITH: The operator matches if the field value ends with the specified value.
CONTAINS: The operator matches if the field value contains the specified value.
EQUALS_ANY: The operator matches if the field value is any value. Possible values: ["CONTAINS", "ENDS_WITH", "EQUALS", "EQUALS_ANY", "STARTS_WITH"]</rdfs:comment>
    <rdfs:domain rdf:resource="http://example.org/onto/class/google_compute_region_security_policy"/>
    <rdfs:range rdf:resource="http://www.w3.org/2001/XMLSchema#string"/>
  </owl:DatatypeProperty>
  <owl:DatatypeProperty rdf:about="http://example.org/onto/prop/google_compute_region_security_policy_value">
    <rdfs:label>value</rdfs:label>
    <rdfs:comment>A request field matching the specified value will be excluded from inspection during preconfigured WAF evaluation.
The field value must be given if the field operator is not EQUALS_ANY, and cannot be given if the field operator is EQUALS_ANY.</rdfs:comment>
    <rdfs:domain rdf:resource="http://example.org/onto/class/google_compute_region_security_policy"/>
    <rdfs:range rdf:resource="http://www.w3.org/2001/XMLSchema#string"/>
  </owl:DatatypeProperty>
  <owl:DatatypeProperty rdf:about="http://example.org/onto/prop/google_compute_region_security_policy_ban_duration_sec">
    <rdfs:label>ban_duration_sec</rdfs:label>
    <rdfs:comment>Can only be specified if the action for the rule is "rate_based_ban".
If specified, determines the time (in seconds) the traffic will continue to be banned by the rate limit after the rate falls below the threshold.</rdfs:comment>
    <rdfs:domain rdf:resource="http://example.org/onto/class/google_compute_region_security_policy"/>
    <rdfs:range rdf:resource="http://www.w3.org/2001/XMLSchema#string"/>
  </owl:DatatypeProperty>
  <owl:DatatypeProperty rdf:about="http://example.org/onto/prop/google_compute_region_security_policy_conform_action">
    <rdfs:label>conform_action</rdfs:label>
    <rdfs:comment>Action to take for requests that are under the configured rate limit threshold.
Valid option is "allow" only.</rdfs:comment>
    <rdfs:domain rdf:resource="http://example.org/onto/class/google_compute_region_security_policy"/>
    <rdfs:range rdf:resource="http://www.w3.org/2001/XMLSchema#string"/>
  </owl:DatatypeProperty>
  <owl:DatatypeProperty rdf:about="http://example.org/onto/prop/google_compute_region_security_policy_enforce_on_key">
    <rdfs:label>enforce_on_key</rdfs:label>
    <rdfs:comment>Determines the key to enforce the rateLimitThreshold on. Possible values are:
* ALL: A single rate limit threshold is applied to all the requests matching this rule. This is the default value if "enforceOnKey" is not configured.
* IP: The source IP address of the request is the key. Each IP has this limit enforced separately.
* HTTP_HEADER: The value of the HTTP header whose name is configured under "enforceOnKeyName". The key value is truncated to the first 128 bytes of the header value. If no such header is present in the request, the key type defaults to ALL.
* XFF_IP: The first IP address (i.e. the originating client IP address) specified in the list of IPs under X-Forwarded-For HTTP header. If no such header is present or the value is not a valid IP, the key defaults to the source IP address of the request i.e. key type IP.
* HTTP_COOKIE: The value of the HTTP cookie whose name is configured under "enforceOnKeyName". The key value is truncated to the first 128 bytes of the cookie value. If no such cookie is present in the request, the key type defaults to ALL.
* HTTP_PATH: The URL path of the HTTP request. The key value is truncated to the first 128 bytes.
* SNI: Server name indication in the TLS session of the HTTPS request. The key value is truncated to the first 128 bytes. The key type defaults to ALL on a HTTP session.
* REGION_CODE: The country/region from which the request originates.
* TLS_JA3_FINGERPRINT: JA3 TLS/SSL fingerprint if the client connects using HTTPS, HTTP/2 or HTTP/3. If not available, the key type defaults to ALL.
* TLS_JA4_FINGERPRINT: JA4 TLS/SSL fingerprint if the client connects using HTTPS, HTTP/2 or HTTP/3. If not available, the key type defaults to ALL.
* USER_IP: The IP address of the originating client, which is resolved based on "userIpRequestHeaders" configured with the security policy. If there is no "userIpRequestHeaders" configuration or an IP address cannot be resolved from it, the key type defaults to IP. Possible values: ["ALL", "IP", "HTTP_HEADER", "XFF_IP", "HTTP_COOKIE", "HTTP_PATH", "SNI", "REGION_CODE", "TLS_JA3_FINGERPRINT", "TLS_JA4_FINGERPRINT", "USER_IP"]</rdfs:comment>
    <rdfs:domain rdf:resource="http://example.org/onto/class/google_compute_region_security_policy"/>
    <rdfs:range rdf:resource="http://www.w3.org/2001/XMLSchema#string"/>
  </owl:DatatypeProperty>
  <owl:DatatypeProperty rdf:about="http://example.org/onto/prop/google_compute_region_security_policy_enforce_on_key_name">
    <rdfs:label>enforce_on_key_name</rdfs:label>
    <rdfs:comment>Rate limit key name applicable only for the following key types:
HTTP_HEADER -- Name of the HTTP header whose value is taken as the key value.
HTTP_COOKIE -- Name of the HTTP cookie whose value is taken as the key value.</rdfs:comment>
    <rdfs:domain rdf:resource="http://example.org/onto/class/google_compute_region_security_policy"/>
    <rdfs:range rdf:resource="http://www.w3.org/2001/XMLSchema#string"/>
  </owl:DatatypeProperty>
  <owl:DatatypeProperty rdf:about="http://example.org/onto/prop/google_compute_region_security_policy_exceed_action">
    <rdfs:label>exceed_action</rdfs:label>
    <rdfs:comment>Action to take for requests that are above the configured rate limit threshold, to deny with a specified HTTP response code.
Valid options are deny(STATUS), where valid values for STATUS are 403, 404, 429, and 502.</rdfs:comment>
    <rdfs:domain rdf:resource="http://example.org/onto/class/google_compute_region_security_policy"/>
    <rdfs:range rdf:resource="http://www.w3.org/2001/XMLSchema#string"/>
  </owl:DatatypeProperty>
  <owl:DatatypeProperty rdf:about="http://example.org/onto/prop/google_compute_region_security_policy_count">
    <rdfs:label>count</rdfs:label>
    <rdfs:comment>Number of HTTP(S) requests for calculating the threshold.</rdfs:comment>
    <rdfs:domain rdf:resource="http://example.org/onto/class/google_compute_region_security_policy"/>
    <rdfs:range rdf:resource="http://www.w3.org/2001/XMLSchema#string"/>
  </owl:DatatypeProperty>
  <owl:DatatypeProperty rdf:about="http://example.org/onto/prop/google_compute_region_security_policy_interval_sec">
    <rdfs:label>interval_sec</rdfs:label>
    <rdfs:comment>Interval over which the threshold is computed.</rdfs:comment>
    <rdfs:domain rdf:resource="http://example.org/onto/class/google_compute_region_security_policy"/>
    <rdfs:range rdf:resource="http://www.w3.org/2001/XMLSchema#string"/>
  </owl:DatatypeProperty>
  <owl:DatatypeProperty rdf:about="http://example.org/onto/prop/google_compute_region_security_policy_enforce_on_key_name">
    <rdfs:label>enforce_on_key_name</rdfs:label>
    <rdfs:comment>Rate limit key name applicable only for the following key types:
HTTP_HEADER -- Name of the HTTP header whose value is taken as the key value.
HTTP_COOKIE -- Name of the HTTP cookie whose value is taken as the key value.</rdfs:comment>
    <rdfs:domain rdf:resource="http://example.org/onto/class/google_compute_region_security_policy"/>
    <rdfs:range rdf:resource="http://www.w3.org/2001/XMLSchema#string"/>
  </owl:DatatypeProperty>
  <owl:DatatypeProperty rdf:about="http://example.org/onto/prop/google_compute_region_security_policy_enforce_on_key_type">
    <rdfs:label>enforce_on_key_type</rdfs:label>
    <rdfs:comment>Determines the key to enforce the rateLimitThreshold on. Possible values are:
* ALL: A single rate limit threshold is applied to all the requests matching this rule. This is the default value if "enforceOnKeyConfigs" is not configured.
* IP: The source IP address of the request is the key. Each IP has this limit enforced separately.
* HTTP_HEADER: The value of the HTTP header whose name is configured under "enforceOnKeyName". The key value is truncated to the first 128 bytes of the header value. If no such header is present in the request, the key type defaults to ALL.
* XFF_IP: The first IP address (i.e. the originating client IP address) specified in the list of IPs under X-Forwarded-For HTTP header. If no such header is present or the value is not a valid IP, the key defaults to the source IP address of the request i.e. key type IP.
* HTTP_COOKIE: The value of the HTTP cookie whose name is configured under "enforceOnKeyName". The key value is truncated to the first 128 bytes of the cookie value. If no such cookie is present in the request, the key type defaults to ALL.
* HTTP_PATH: The URL path of the HTTP request. The key value is truncated to the first 128 bytes.
* SNI: Server name indication in the TLS session of the HTTPS request. The key value is truncated to the first 128 bytes. The key type defaults to ALL on a HTTP session.
* REGION_CODE: The country/region from which the request originates.
* TLS_JA3_FINGERPRINT: JA3 TLS/SSL fingerprint if the client connects using HTTPS, HTTP/2 or HTTP/3. If not available, the key type defaults to ALL.
* TLS_JA4_FINGERPRINT: JA4 TLS/SSL fingerprint if the client connects using HTTPS, HTTP/2 or HTTP/3. If not available, the key type defaults to ALL.
* USER_IP: The IP address of the originating client, which is resolved based on "userIpRequestHeaders" configured with the security policy. If there is no "userIpRequestHeaders" configuration or an IP address cannot be resolved from it, the key type defaults to IP. Possible values: ["ALL", "IP", "HTTP_HEADER", "XFF_IP", "HTTP_COOKIE", "HTTP_PATH", "SNI", "REGION_CODE", "TLS_JA3_FINGERPRINT", "TLS_JA4_FINGERPRINT", "USER_IP"]</rdfs:comment>
    <rdfs:domain rdf:resource="http://example.org/onto/class/google_compute_region_security_policy"/>
    <rdfs:range rdf:resource="http://www.w3.org/2001/XMLSchema#string"/>
  </owl:DatatypeProperty>
  <owl:DatatypeProperty rdf:about="http://example.org/onto/prop/google_compute_region_security_policy_count">
    <rdfs:label>count</rdfs:label>
    <rdfs:comment>Number of HTTP(S) requests for calculating the threshold.</rdfs:comment>
    <rdfs:domain rdf:resource="http://example.org/onto/class/google_compute_region_security_policy"/>
    <rdfs:range rdf:resource="http://www.w3.org/2001/XMLSchema#string"/>
  </owl:DatatypeProperty>
  <owl:DatatypeProperty rdf:about="http://example.org/onto/prop/google_compute_region_security_policy_interval_sec">
    <rdfs:label>interval_sec</rdfs:label>
    <rdfs:comment>Interval over which the threshold is computed.</rdfs:comment>
    <rdfs:domain rdf:resource="http://example.org/onto/class/google_compute_region_security_policy"/>
    <rdfs:range rdf:resource="http://www.w3.org/2001/XMLSchema#string"/>
  </owl:DatatypeProperty>
  <owl:DatatypeProperty rdf:about="http://example.org/onto/prop/google_compute_region_security_policy_create">
    <rdfs:label>create</rdfs:label>
    <rdfs:domain rdf:resource="http://example.org/onto/class/google_compute_region_security_policy"/>
    <rdfs:range rdf:resource="http://www.w3.org/2001/XMLSchema#string"/>
  </owl:DatatypeProperty>
  <owl:DatatypeProperty rdf:about="http://example.org/onto/prop/google_compute_region_security_policy_delete">
    <rdfs:label>delete</rdfs:label>
    <rdfs:domain rdf:resource="http://example.org/onto/class/google_compute_region_security_policy"/>
    <rdfs:range rdf:resource="http://www.w3.org/2001/XMLSchema#string"/>
  </owl:DatatypeProperty>
  <owl:DatatypeProperty rdf:about="http://example.org/onto/prop/google_compute_region_security_policy_update">
    <rdfs:label>update</rdfs:label>
    <rdfs:domain rdf:resource="http://example.org/onto/class/google_compute_region_security_policy"/>
    <rdfs:range rdf:resource="http://www.w3.org/2001/XMLSchema#string"/>
  </owl:DatatypeProperty>
  <owl:DatatypeProperty rdf:about="http://example.org/onto/prop/google_compute_region_security_policy_base">
    <rdfs:label>base</rdfs:label>
    <rdfs:comment>The base relative to which 'offset' is measured. Possible values are:
- IPV4: Points to the beginning of the IPv4 header.
- IPV6: Points to the beginning of the IPv6 header.
- TCP: Points to the beginning of the TCP header, skipping over any IPv4 options or IPv6 extension headers. Not present for non-first fragments.
- UDP: Points to the beginning of the UDP header, skipping over any IPv4 options or IPv6 extension headers. Not present for non-first fragments. Possible values: ["IPV4", "IPV6", "TCP", "UDP"]</rdfs:comment>
    <rdfs:domain rdf:resource="http://example.org/onto/class/google_compute_region_security_policy"/>
    <rdfs:range rdf:resource="http://www.w3.org/2001/XMLSchema#string"/>
  </owl:DatatypeProperty>
  <owl:DatatypeProperty rdf:about="http://example.org/onto/prop/google_compute_region_security_policy_mask">
    <rdfs:label>mask</rdfs:label>
    <rdfs:comment>If specified, apply this mask (bitwise AND) to the field to ignore bits before matching.
Encoded as a hexadecimal number (starting with "0x").
The last byte of the field (in network byte order) corresponds to the least significant byte of the mask.</rdfs:comment>
    <rdfs:domain rdf:resource="http://example.org/onto/class/google_compute_region_security_policy"/>
    <rdfs:range rdf:resource="http://www.w3.org/2001/XMLSchema#string"/>
  </owl:DatatypeProperty>
  <owl:DatatypeProperty rdf:about="http://example.org/onto/prop/google_compute_region_security_policy_name">
    <rdfs:label>name</rdfs:label>
    <rdfs:comment>The name of this field. Must be unique within the policy.</rdfs:comment>
    <rdfs:domain rdf:resource="http://example.org/onto/class/google_compute_region_security_policy"/>
    <rdfs:range rdf:resource="http://www.w3.org/2001/XMLSchema#string"/>
  </owl:DatatypeProperty>
  <owl:DatatypeProperty rdf:about="http://example.org/onto/prop/google_compute_region_security_policy_offset">
    <rdfs:label>offset</rdfs:label>
    <rdfs:comment>Offset of the first byte of the field (in network byte order) relative to 'base'.</rdfs:comment>
    <rdfs:domain rdf:resource="http://example.org/onto/class/google_compute_region_security_policy"/>
    <rdfs:range rdf:resource="http://www.w3.org/2001/XMLSchema#string"/>
  </owl:DatatypeProperty>
  <owl:DatatypeProperty rdf:about="http://example.org/onto/prop/google_compute_region_security_policy_size">
    <rdfs:label>size</rdfs:label>
    <rdfs:comment>Size of the field in bytes. Valid values: 1-4.</rdfs:comment>
    <rdfs:domain rdf:resource="http://example.org/onto/class/google_compute_region_security_policy"/>
    <rdfs:range rdf:resource="http://www.w3.org/2001/XMLSchema#string"/>
  </owl:DatatypeProperty>
</rdf:RDF>
