<?xml version="1.0" encoding="UTF-8"?>
<rdf:RDF
  xmlns:rdf="http://www.w3.org/1999/02/22-rdf-syntax-ns#"
  xmlns:rdfs="http://www.w3.org/2000/01/rdf-schema#"
  xmlns:owl="http://www.w3.org/2002/07/owl#"
  xmlns:xsd="http://www.w3.org/2001/XMLSchema#"
  xml:base="http://example.org/onto/">
  <owl:Class rdf:about="http://example.org/onto/class/google_compute_service_attachment">
    <rdfs:label>google_compute_service_attachment</rdfs:label>
    <rdfs:comment>#
#     ***     AUTO GENERATED CODE    ***    Type: MMv1     ***
#
# ----------------------------------------------------------------------------
#
#     This code is generated by Magic Modules using the following:
#
#     Configuration: https:#github.com/GoogleCloudPlatform/magic-modules/tree/main/mmv1/products/compute/ServiceAttachment.yaml
#     Template:      https:#github.com/GoogleCloudPlatform/magic-modules/tree/main/mmv1/templates/terraform/resource.html.markdown.tmpl
#
#     DO NOT EDIT this file directly. Any changes made to this file will be
#     overwritten during the next generation cycle.
#
# ----------------------------------------------------------------------------
subcategory: "Compute Engine"
description: |-
  Represents a ServiceAttachment resource.
---</rdfs:comment>
  </owl:Class>
  <owl:DatatypeProperty rdf:about="http://example.org/onto/prop/google_compute_service_attachment_connected_endpoints">
    <rdfs:label>connected_endpoints</rdfs:label>
    <rdfs:comment>An array of the consumer forwarding rules connected to this service
attachment.</rdfs:comment>
    <rdfs:domain rdf:resource="http://example.org/onto/class/google_compute_service_attachment"/>
    <rdfs:range rdf:resource="http://www.w3.org/2001/XMLSchema#string"/>
  </owl:DatatypeProperty>
  <owl:DatatypeProperty rdf:about="http://example.org/onto/prop/google_compute_service_attachment_connection_preference">
    <rdfs:label>connection_preference</rdfs:label>
    <rdfs:comment>The connection preference to use for this service attachment. Valid
values include "ACCEPT_AUTOMATIC", "ACCEPT_MANUAL".</rdfs:comment>
    <rdfs:domain rdf:resource="http://example.org/onto/class/google_compute_service_attachment"/>
    <rdfs:range rdf:resource="http://www.w3.org/2001/XMLSchema#string"/>
  </owl:DatatypeProperty>
  <owl:DatatypeProperty rdf:about="http://example.org/onto/prop/google_compute_service_attachment_consumer_reject_lists">
    <rdfs:label>consumer_reject_lists</rdfs:label>
    <rdfs:comment>An array of projects that are not allowed to connect to this service
attachment.</rdfs:comment>
    <rdfs:domain rdf:resource="http://example.org/onto/class/google_compute_service_attachment"/>
    <rdfs:range rdf:resource="http://www.w3.org/2001/XMLSchema#string"/>
  </owl:DatatypeProperty>
  <owl:DatatypeProperty rdf:about="http://example.org/onto/prop/google_compute_service_attachment_description">
    <rdfs:label>description</rdfs:label>
    <rdfs:comment>An optional description of this resource.</rdfs:comment>
    <rdfs:domain rdf:resource="http://example.org/onto/class/google_compute_service_attachment"/>
    <rdfs:range rdf:resource="http://www.w3.org/2001/XMLSchema#string"/>
  </owl:DatatypeProperty>
  <owl:DatatypeProperty rdf:about="http://example.org/onto/prop/google_compute_service_attachment_domain_names">
    <rdfs:label>domain_names</rdfs:label>
    <rdfs:comment>If specified, the domain name will be used during the integration between
the PSC connected endpoints and the Cloud DNS. For example, this is a
valid domain name: "p.mycompany.com.". Current max number of domain names
supported is 1.</rdfs:comment>
    <rdfs:domain rdf:resource="http://example.org/onto/class/google_compute_service_attachment"/>
    <rdfs:range rdf:resource="http://www.w3.org/2001/XMLSchema#string"/>
  </owl:DatatypeProperty>
  <owl:DatatypeProperty rdf:about="http://example.org/onto/prop/google_compute_service_attachment_enable_proxy_protocol">
    <rdfs:label>enable_proxy_protocol</rdfs:label>
    <rdfs:comment>If true, enable the proxy protocol which is for supplying client TCP/IP
address data in TCP connections that traverse proxies on their way to
destination servers.</rdfs:comment>
    <rdfs:domain rdf:resource="http://example.org/onto/class/google_compute_service_attachment"/>
    <rdfs:range rdf:resource="http://www.w3.org/2001/XMLSchema#string"/>
  </owl:DatatypeProperty>
  <owl:DatatypeProperty rdf:about="http://example.org/onto/prop/google_compute_service_attachment_fingerprint">
    <rdfs:label>fingerprint</rdfs:label>
    <rdfs:comment>Fingerprint of this resource. This field is used internally during
updates of this resource.</rdfs:comment>
    <rdfs:domain rdf:resource="http://example.org/onto/class/google_compute_service_attachment"/>
    <rdfs:range rdf:resource="http://www.w3.org/2001/XMLSchema#string"/>
  </owl:DatatypeProperty>
  <owl:DatatypeProperty rdf:about="http://example.org/onto/prop/google_compute_service_attachment_id">
    <rdfs:label>id</rdfs:label>
    <rdfs:domain rdf:resource="http://example.org/onto/class/google_compute_service_attachment"/>
    <rdfs:range rdf:resource="http://www.w3.org/2001/XMLSchema#string"/>
  </owl:DatatypeProperty>
  <owl:DatatypeProperty rdf:about="http://example.org/onto/prop/google_compute_service_attachment_name">
    <rdfs:label>name</rdfs:label>
    <rdfs:comment>Name of the resource. The name must be 1-63 characters long, and
comply with RFC1035. Specifically, the name must be 1-63 characters
long and match the regular expression '[a-z]([-a-z0-9]*[a-z0-9])?'
which means the first character must be a lowercase letter, and all
following characters must be a dash, lowercase letter, or digit,
except the last character, which cannot be a dash.</rdfs:comment>
    <rdfs:domain rdf:resource="http://example.org/onto/class/google_compute_service_attachment"/>
    <rdfs:range rdf:resource="http://www.w3.org/2001/XMLSchema#string"/>
  </owl:DatatypeProperty>
  <owl:DatatypeProperty rdf:about="http://example.org/onto/prop/google_compute_service_attachment_nat_subnets">
    <rdfs:label>nat_subnets</rdfs:label>
    <rdfs:comment>An array of subnets that is provided for NAT in this service attachment.</rdfs:comment>
    <rdfs:domain rdf:resource="http://example.org/onto/class/google_compute_service_attachment"/>
    <rdfs:range rdf:resource="http://www.w3.org/2001/XMLSchema#string"/>
  </owl:DatatypeProperty>
  <owl:DatatypeProperty rdf:about="http://example.org/onto/prop/google_compute_service_attachment_project">
    <rdfs:label>project</rdfs:label>
    <rdfs:domain rdf:resource="http://example.org/onto/class/google_compute_service_attachment"/>
    <rdfs:range rdf:resource="http://www.w3.org/2001/XMLSchema#string"/>
  </owl:DatatypeProperty>
  <owl:DatatypeProperty rdf:about="http://example.org/onto/prop/google_compute_service_attachment_propagated_connection_limit">
    <rdfs:label>propagated_connection_limit</rdfs:label>
    <rdfs:comment>The number of consumer spokes that connected Private Service Connect endpoints can be propagated to through Network Connectivity Center.
This limit lets the service producer limit how many propagated Private Service Connect connections can be established to this service attachment from a single consumer.

If the connection preference of the service attachment is ACCEPT_MANUAL, the limit applies to each project or network that is listed in the consumer accept list.
If the connection preference of the service attachment is ACCEPT_AUTOMATIC, the limit applies to each project that contains a connected endpoint.

If unspecified, the default propagated connection limit is 250. To explicitly send a zero value, set 'send_propagated_connection_limit_if_zero = true'.</rdfs:comment>
    <rdfs:domain rdf:resource="http://example.org/onto/class/google_compute_service_attachment"/>
    <rdfs:range rdf:resource="http://www.w3.org/2001/XMLSchema#string"/>
  </owl:DatatypeProperty>
  <owl:DatatypeProperty rdf:about="http://example.org/onto/prop/google_compute_service_attachment_psc_service_attachment_id">
    <rdfs:label>psc_service_attachment_id</rdfs:label>
    <rdfs:comment>An 128-bit global unique ID of the PSC service attachment.</rdfs:comment>
    <rdfs:domain rdf:resource="http://example.org/onto/class/google_compute_service_attachment"/>
    <rdfs:range rdf:resource="http://www.w3.org/2001/XMLSchema#string"/>
  </owl:DatatypeProperty>
  <owl:DatatypeProperty rdf:about="http://example.org/onto/prop/google_compute_service_attachment_reconcile_connections">
    <rdfs:label>reconcile_connections</rdfs:label>
    <rdfs:comment>This flag determines whether a consumer accept/reject list change can reconcile the statuses of existing ACCEPTED or REJECTED PSC endpoints.

If false, connection policy update will only affect existing PENDING PSC endpoints. Existing ACCEPTED/REJECTED endpoints will remain untouched regardless how the connection policy is modified .
If true, update will affect both PENDING and ACCEPTED/REJECTED PSC endpoints. For example, an ACCEPTED PSC endpoint will be moved to REJECTED if its project is added to the reject list.</rdfs:comment>
    <rdfs:domain rdf:resource="http://example.org/onto/class/google_compute_service_attachment"/>
    <rdfs:range rdf:resource="http://www.w3.org/2001/XMLSchema#string"/>
  </owl:DatatypeProperty>
  <owl:DatatypeProperty rdf:about="http://example.org/onto/prop/google_compute_service_attachment_region">
    <rdfs:label>region</rdfs:label>
    <rdfs:comment>URL of the region where the resource resides.</rdfs:comment>
    <rdfs:domain rdf:resource="http://example.org/onto/class/google_compute_service_attachment"/>
    <rdfs:range rdf:resource="http://www.w3.org/2001/XMLSchema#string"/>
  </owl:DatatypeProperty>
  <owl:DatatypeProperty rdf:about="http://example.org/onto/prop/google_compute_service_attachment_self_link">
    <rdfs:label>self_link</rdfs:label>
    <rdfs:domain rdf:resource="http://example.org/onto/class/google_compute_service_attachment"/>
    <rdfs:range rdf:resource="http://www.w3.org/2001/XMLSchema#string"/>
  </owl:DatatypeProperty>
  <owl:DatatypeProperty rdf:about="http://example.org/onto/prop/google_compute_service_attachment_send_propagated_connection_limit_if_zero">
    <rdfs:label>send_propagated_connection_limit_if_zero</rdfs:label>
    <rdfs:comment>Controls the behavior of propagated_connection_limit.
When false, setting propagated_connection_limit to zero causes the provider to use to the API's default value.
When true, the provider will set propagated_connection_limit to zero.
Defaults to false.</rdfs:comment>
    <rdfs:domain rdf:resource="http://example.org/onto/class/google_compute_service_attachment"/>
    <rdfs:range rdf:resource="http://www.w3.org/2001/XMLSchema#string"/>
  </owl:DatatypeProperty>
  <owl:DatatypeProperty rdf:about="http://example.org/onto/prop/google_compute_service_attachment_target_service">
    <rdfs:label>target_service</rdfs:label>
    <rdfs:comment>The URL of a service serving the endpoint identified by this service attachment.</rdfs:comment>
    <rdfs:domain rdf:resource="http://example.org/onto/class/google_compute_service_attachment"/>
    <rdfs:range rdf:resource="http://www.w3.org/2001/XMLSchema#string"/>
  </owl:DatatypeProperty>
  <owl:DatatypeProperty rdf:about="http://example.org/onto/prop/google_compute_service_attachment_connection_limit">
    <rdfs:label>connection_limit</rdfs:label>
    <rdfs:comment>The number of consumer forwarding rules the consumer project can
create.</rdfs:comment>
    <rdfs:domain rdf:resource="http://example.org/onto/class/google_compute_service_attachment"/>
    <rdfs:range rdf:resource="http://www.w3.org/2001/XMLSchema#string"/>
  </owl:DatatypeProperty>
  <owl:DatatypeProperty rdf:about="http://example.org/onto/prop/google_compute_service_attachment_network_url">
    <rdfs:label>network_url</rdfs:label>
    <rdfs:comment>The network that is allowed to connect to this service attachment.
Only one of project_id_or_num and network_url may be set.</rdfs:comment>
    <rdfs:domain rdf:resource="http://example.org/onto/class/google_compute_service_attachment"/>
    <rdfs:range rdf:resource="http://www.w3.org/2001/XMLSchema#string"/>
  </owl:DatatypeProperty>
  <owl:DatatypeProperty rdf:about="http://example.org/onto/prop/google_compute_service_attachment_project_id_or_num">
    <rdfs:label>project_id_or_num</rdfs:label>
    <rdfs:comment>A project that is allowed to connect to this service attachment.
Only one of project_id_or_num and network_url may be set.</rdfs:comment>
    <rdfs:domain rdf:resource="http://example.org/onto/class/google_compute_service_attachment"/>
    <rdfs:range rdf:resource="http://www.w3.org/2001/XMLSchema#string"/>
  </owl:DatatypeProperty>
  <owl:DatatypeProperty rdf:about="http://example.org/onto/prop/google_compute_service_attachment_create">
    <rdfs:label>create</rdfs:label>
    <rdfs:domain rdf:resource="http://example.org/onto/class/google_compute_service_attachment"/>
    <rdfs:range rdf:resource="http://www.w3.org/2001/XMLSchema#string"/>
  </owl:DatatypeProperty>
  <owl:DatatypeProperty rdf:about="http://example.org/onto/prop/google_compute_service_attachment_delete">
    <rdfs:label>delete</rdfs:label>
    <rdfs:domain rdf:resource="http://example.org/onto/class/google_compute_service_attachment"/>
    <rdfs:range rdf:resource="http://www.w3.org/2001/XMLSchema#string"/>
  </owl:DatatypeProperty>
  <owl:DatatypeProperty rdf:about="http://example.org/onto/prop/google_compute_service_attachment_update">
    <rdfs:label>update</rdfs:label>
    <rdfs:domain rdf:resource="http://example.org/onto/class/google_compute_service_attachment"/>
    <rdfs:range rdf:resource="http://www.w3.org/2001/XMLSchema#string"/>
  </owl:DatatypeProperty>
</rdf:RDF>
