<?xml version="1.0" encoding="UTF-8"?>
<rdf:RDF
  xmlns:rdf="http://www.w3.org/1999/02/22-rdf-syntax-ns#"
  xmlns:rdfs="http://www.w3.org/2000/01/rdf-schema#"
  xmlns:owl="http://www.w3.org/2002/07/owl#"
  xmlns:xsd="http://www.w3.org/2001/XMLSchema#"
  xml:base="http://example.org/onto/">
  <owl:Class rdf:about="http://example.org/onto/class/google_vertex_ai_index_endpoint">
    <rdfs:label>google_vertex_ai_index_endpoint</rdfs:label>
    <rdfs:comment>#
#     ***     AUTO GENERATED CODE    ***    Type: MMv1     ***
#
# ----------------------------------------------------------------------------
#
#     This code is generated by Magic Modules using the following:
#
#     Configuration: https:#github.com/GoogleCloudPlatform/magic-modules/tree/main/mmv1/products/vertexai/IndexEndpoint.yaml
#     Template:      https:#github.com/GoogleCloudPlatform/magic-modules/tree/main/mmv1/templates/terraform/resource.html.markdown.tmpl
#
#     DO NOT EDIT this file directly. Any changes made to this file will be
#     overwritten during the next generation cycle.
#
# ----------------------------------------------------------------------------
subcategory: "Vertex AI"
description: |-
  An endpoint indexes are deployed into.
---</rdfs:comment>
  </owl:Class>
  <owl:DatatypeProperty rdf:about="http://example.org/onto/prop/google_vertex_ai_index_endpoint_create_time">
    <rdfs:label>create_time</rdfs:label>
    <rdfs:comment>The timestamp of when the Index was created in RFC3339 UTC "Zulu" format, with nanosecond resolution and up to nine fractional digits.</rdfs:comment>
    <rdfs:domain rdf:resource="http://example.org/onto/class/google_vertex_ai_index_endpoint"/>
    <rdfs:range rdf:resource="http://www.w3.org/2001/XMLSchema#string"/>
  </owl:DatatypeProperty>
  <owl:DatatypeProperty rdf:about="http://example.org/onto/prop/google_vertex_ai_index_endpoint_description">
    <rdfs:label>description</rdfs:label>
    <rdfs:comment>The description of the Index.</rdfs:comment>
    <rdfs:domain rdf:resource="http://example.org/onto/class/google_vertex_ai_index_endpoint"/>
    <rdfs:range rdf:resource="http://www.w3.org/2001/XMLSchema#string"/>
  </owl:DatatypeProperty>
  <owl:DatatypeProperty rdf:about="http://example.org/onto/prop/google_vertex_ai_index_endpoint_display_name">
    <rdfs:label>display_name</rdfs:label>
    <rdfs:comment>The display name of the Index. The name can be up to 128 characters long and can consist of any UTF-8 characters.</rdfs:comment>
    <rdfs:domain rdf:resource="http://example.org/onto/class/google_vertex_ai_index_endpoint"/>
    <rdfs:range rdf:resource="http://www.w3.org/2001/XMLSchema#string"/>
  </owl:DatatypeProperty>
  <owl:DatatypeProperty rdf:about="http://example.org/onto/prop/google_vertex_ai_index_endpoint_effective_labels">
    <rdfs:label>effective_labels</rdfs:label>
    <rdfs:comment>All of labels (key/value pairs) present on the resource in GCP, including the labels configured through Terraform, other clients and services.</rdfs:comment>
    <rdfs:domain rdf:resource="http://example.org/onto/class/google_vertex_ai_index_endpoint"/>
    <rdfs:range rdf:resource="http://www.w3.org/2001/XMLSchema#string"/>
  </owl:DatatypeProperty>
  <owl:DatatypeProperty rdf:about="http://example.org/onto/prop/google_vertex_ai_index_endpoint_etag">
    <rdfs:label>etag</rdfs:label>
    <rdfs:comment>Used to perform consistent read-modify-write updates.</rdfs:comment>
    <rdfs:domain rdf:resource="http://example.org/onto/class/google_vertex_ai_index_endpoint"/>
    <rdfs:range rdf:resource="http://www.w3.org/2001/XMLSchema#string"/>
  </owl:DatatypeProperty>
  <owl:DatatypeProperty rdf:about="http://example.org/onto/prop/google_vertex_ai_index_endpoint_id">
    <rdfs:label>id</rdfs:label>
    <rdfs:domain rdf:resource="http://example.org/onto/class/google_vertex_ai_index_endpoint"/>
    <rdfs:range rdf:resource="http://www.w3.org/2001/XMLSchema#string"/>
  </owl:DatatypeProperty>
  <owl:DatatypeProperty rdf:about="http://example.org/onto/prop/google_vertex_ai_index_endpoint_labels">
    <rdfs:label>labels</rdfs:label>
    <rdfs:comment>The labels with user-defined metadata to organize your Indexes.

**Note**: This field is non-authoritative, and will only manage the labels present in your configuration.
Please refer to the field 'effective_labels' for all of the labels present on the resource.</rdfs:comment>
    <rdfs:domain rdf:resource="http://example.org/onto/class/google_vertex_ai_index_endpoint"/>
    <rdfs:range rdf:resource="http://www.w3.org/2001/XMLSchema#string"/>
  </owl:DatatypeProperty>
  <owl:DatatypeProperty rdf:about="http://example.org/onto/prop/google_vertex_ai_index_endpoint_name">
    <rdfs:label>name</rdfs:label>
    <rdfs:comment>The resource name of the Index.</rdfs:comment>
    <rdfs:domain rdf:resource="http://example.org/onto/class/google_vertex_ai_index_endpoint"/>
    <rdfs:range rdf:resource="http://www.w3.org/2001/XMLSchema#string"/>
  </owl:DatatypeProperty>
  <owl:DatatypeProperty rdf:about="http://example.org/onto/prop/google_vertex_ai_index_endpoint_network">
    <rdfs:label>network</rdfs:label>
    <rdfs:comment>The full name of the Google Compute Engine [network](https://cloud.google.com//compute/docs/networks-and-firewalls#networks) to which the index endpoint should be peered.
Private services access must already be configured for the network. If left unspecified, the index endpoint is not peered with any network.
[Format](https://cloud.google.com/compute/docs/reference/rest/v1/networks/insert): 'projects/{project}/global/networks/{network}'.
Where '{project}' is a project number, as in '12345', and '{network}' is network name.</rdfs:comment>
    <rdfs:domain rdf:resource="http://example.org/onto/class/google_vertex_ai_index_endpoint"/>
    <rdfs:range rdf:resource="http://www.w3.org/2001/XMLSchema#string"/>
  </owl:DatatypeProperty>
  <owl:DatatypeProperty rdf:about="http://example.org/onto/prop/google_vertex_ai_index_endpoint_project">
    <rdfs:label>project</rdfs:label>
    <rdfs:domain rdf:resource="http://example.org/onto/class/google_vertex_ai_index_endpoint"/>
    <rdfs:range rdf:resource="http://www.w3.org/2001/XMLSchema#string"/>
  </owl:DatatypeProperty>
  <owl:DatatypeProperty rdf:about="http://example.org/onto/prop/google_vertex_ai_index_endpoint_public_endpoint_domain_name">
    <rdfs:label>public_endpoint_domain_name</rdfs:label>
    <rdfs:comment>If publicEndpointEnabled is true, this field will be populated with the domain name to use for this index endpoint.</rdfs:comment>
    <rdfs:domain rdf:resource="http://example.org/onto/class/google_vertex_ai_index_endpoint"/>
    <rdfs:range rdf:resource="http://www.w3.org/2001/XMLSchema#string"/>
  </owl:DatatypeProperty>
  <owl:DatatypeProperty rdf:about="http://example.org/onto/prop/google_vertex_ai_index_endpoint_public_endpoint_enabled">
    <rdfs:label>public_endpoint_enabled</rdfs:label>
    <rdfs:comment>If true, the deployed index will be accessible through public endpoint.</rdfs:comment>
    <rdfs:domain rdf:resource="http://example.org/onto/class/google_vertex_ai_index_endpoint"/>
    <rdfs:range rdf:resource="http://www.w3.org/2001/XMLSchema#string"/>
  </owl:DatatypeProperty>
  <owl:DatatypeProperty rdf:about="http://example.org/onto/prop/google_vertex_ai_index_endpoint_region">
    <rdfs:label>region</rdfs:label>
    <rdfs:comment>The region of the index endpoint. eg us-central1</rdfs:comment>
    <rdfs:domain rdf:resource="http://example.org/onto/class/google_vertex_ai_index_endpoint"/>
    <rdfs:range rdf:resource="http://www.w3.org/2001/XMLSchema#string"/>
  </owl:DatatypeProperty>
  <owl:DatatypeProperty rdf:about="http://example.org/onto/prop/google_vertex_ai_index_endpoint_terraform_labels">
    <rdfs:label>terraform_labels</rdfs:label>
    <rdfs:comment>The combination of labels configured directly on the resource
 and default labels configured on the provider.</rdfs:comment>
    <rdfs:domain rdf:resource="http://example.org/onto/class/google_vertex_ai_index_endpoint"/>
    <rdfs:range rdf:resource="http://www.w3.org/2001/XMLSchema#string"/>
  </owl:DatatypeProperty>
  <owl:DatatypeProperty rdf:about="http://example.org/onto/prop/google_vertex_ai_index_endpoint_update_time">
    <rdfs:label>update_time</rdfs:label>
    <rdfs:comment>The timestamp of when the Index was last updated in RFC3339 UTC "Zulu" format, with nanosecond resolution and up to nine fractional digits.</rdfs:comment>
    <rdfs:domain rdf:resource="http://example.org/onto/class/google_vertex_ai_index_endpoint"/>
    <rdfs:range rdf:resource="http://www.w3.org/2001/XMLSchema#string"/>
  </owl:DatatypeProperty>
  <owl:DatatypeProperty rdf:about="http://example.org/onto/prop/google_vertex_ai_index_endpoint_kms_key_name">
    <rdfs:label>kms_key_name</rdfs:label>
    <rdfs:comment>Required. The Cloud KMS resource identifier of the customer managed encryption key used to protect a resource. Has the form: 'projects/my-project/locations/my-region/keyRings/my-kr/cryptoKeys/my-key'. The key needs to be in the same region as where the compute resource is created.</rdfs:comment>
    <rdfs:domain rdf:resource="http://example.org/onto/class/google_vertex_ai_index_endpoint"/>
    <rdfs:range rdf:resource="http://www.w3.org/2001/XMLSchema#string"/>
  </owl:DatatypeProperty>
  <owl:DatatypeProperty rdf:about="http://example.org/onto/prop/google_vertex_ai_index_endpoint_enable_private_service_connect">
    <rdfs:label>enable_private_service_connect</rdfs:label>
    <rdfs:comment>If set to true, the IndexEndpoint is created without private service access.</rdfs:comment>
    <rdfs:domain rdf:resource="http://example.org/onto/class/google_vertex_ai_index_endpoint"/>
    <rdfs:range rdf:resource="http://www.w3.org/2001/XMLSchema#string"/>
  </owl:DatatypeProperty>
  <owl:DatatypeProperty rdf:about="http://example.org/onto/prop/google_vertex_ai_index_endpoint_project_allowlist">
    <rdfs:label>project_allowlist</rdfs:label>
    <rdfs:comment>A list of Projects from which the forwarding rule will target the service attachment.</rdfs:comment>
    <rdfs:domain rdf:resource="http://example.org/onto/class/google_vertex_ai_index_endpoint"/>
    <rdfs:range rdf:resource="http://www.w3.org/2001/XMLSchema#string"/>
  </owl:DatatypeProperty>
  <owl:DatatypeProperty rdf:about="http://example.org/onto/prop/google_vertex_ai_index_endpoint_create">
    <rdfs:label>create</rdfs:label>
    <rdfs:domain rdf:resource="http://example.org/onto/class/google_vertex_ai_index_endpoint"/>
    <rdfs:range rdf:resource="http://www.w3.org/2001/XMLSchema#string"/>
  </owl:DatatypeProperty>
  <owl:DatatypeProperty rdf:about="http://example.org/onto/prop/google_vertex_ai_index_endpoint_delete">
    <rdfs:label>delete</rdfs:label>
    <rdfs:domain rdf:resource="http://example.org/onto/class/google_vertex_ai_index_endpoint"/>
    <rdfs:range rdf:resource="http://www.w3.org/2001/XMLSchema#string"/>
  </owl:DatatypeProperty>
  <owl:DatatypeProperty rdf:about="http://example.org/onto/prop/google_vertex_ai_index_endpoint_update">
    <rdfs:label>update</rdfs:label>
    <rdfs:domain rdf:resource="http://example.org/onto/class/google_vertex_ai_index_endpoint"/>
    <rdfs:range rdf:resource="http://www.w3.org/2001/XMLSchema#string"/>
  </owl:DatatypeProperty>
</rdf:RDF>
