<?xml version="1.0" encoding="UTF-8"?>
<rdf:RDF
  xmlns:rdf="http://www.w3.org/1999/02/22-rdf-syntax-ns#"
  xmlns:rdfs="http://www.w3.org/2000/01/rdf-schema#"
  xmlns:owl="http://www.w3.org/2002/07/owl#"
  xmlns:xsd="http://www.w3.org/2001/XMLSchema#"
  xml:base="http://example.org/onto/">
  <owl:Class rdf:about="http://example.org/onto/class/google_pubsub_subscription">
    <rdfs:label>google_pubsub_subscription</rdfs:label>
    <rdfs:comment>#
#     ***     AUTO GENERATED CODE    ***    Type: MMv1     ***
#
# ----------------------------------------------------------------------------
#
#     This code is generated by Magic Modules using the following:
#
#     Configuration: https:#github.com/GoogleCloudPlatform/magic-modules/tree/main/mmv1/products/pubsub/Subscription.yaml
#     Template:      https:#github.com/GoogleCloudPlatform/magic-modules/tree/main/mmv1/templates/terraform/resource.html.markdown.tmpl
#
#     DO NOT EDIT this file directly. Any changes made to this file will be
#     overwritten during the next generation cycle.
#
# ----------------------------------------------------------------------------
subcategory: "Cloud Pub/Sub"
description: |-
  A named resource representing the stream of messages from a single,
  specific topic, to be delivered to the subscribing application.
---</rdfs:comment>
  </owl:Class>
  <owl:DatatypeProperty rdf:about="http://example.org/onto/prop/google_pubsub_subscription_ack_deadline_seconds">
    <rdfs:label>ack_deadline_seconds</rdfs:label>
    <rdfs:comment>This value is the maximum time after a subscriber receives a message
before the subscriber should acknowledge the message. After message
delivery but before the ack deadline expires and before the message is
acknowledged, it is an outstanding message and will not be delivered
again during that time (on a best-effort basis).

For pull subscriptions, this value is used as the initial value for
the ack deadline. To override this value for a given message, call
subscriptions.modifyAckDeadline with the corresponding ackId if using
pull. The minimum custom deadline you can specify is 10 seconds. The
maximum custom deadline you can specify is 600 seconds (10 minutes).
If this parameter is 0, a default value of 10 seconds is used.

For push delivery, this value is also used to set the request timeout
for the call to the push endpoint.

If the subscriber never acknowledges the message, the Pub/Sub system
will eventually redeliver the message.</rdfs:comment>
    <rdfs:domain rdf:resource="http://example.org/onto/class/google_pubsub_subscription"/>
    <rdfs:range rdf:resource="http://www.w3.org/2001/XMLSchema#string"/>
  </owl:DatatypeProperty>
  <owl:DatatypeProperty rdf:about="http://example.org/onto/prop/google_pubsub_subscription_effective_labels">
    <rdfs:label>effective_labels</rdfs:label>
    <rdfs:comment>All of labels (key/value pairs) present on the resource in GCP, including the labels configured through Terraform, other clients and services.</rdfs:comment>
    <rdfs:domain rdf:resource="http://example.org/onto/class/google_pubsub_subscription"/>
    <rdfs:range rdf:resource="http://www.w3.org/2001/XMLSchema#string"/>
  </owl:DatatypeProperty>
  <owl:DatatypeProperty rdf:about="http://example.org/onto/prop/google_pubsub_subscription_enable_exactly_once_delivery">
    <rdfs:label>enable_exactly_once_delivery</rdfs:label>
    <rdfs:comment>If 'true', Pub/Sub provides the following guarantees for the delivery
of a message with a given value of messageId on this Subscriptions':

- The message sent to a subscriber is guaranteed not to be resent before the message's acknowledgement deadline expires.

- An acknowledged message will not be resent to a subscriber.

Note that subscribers may still receive multiple copies of a message when 'enable_exactly_once_delivery'
is true if the message was published multiple times by a publisher client. These copies are considered distinct by Pub/Sub and have distinct messageId values</rdfs:comment>
    <rdfs:domain rdf:resource="http://example.org/onto/class/google_pubsub_subscription"/>
    <rdfs:range rdf:resource="http://www.w3.org/2001/XMLSchema#string"/>
  </owl:DatatypeProperty>
  <owl:DatatypeProperty rdf:about="http://example.org/onto/prop/google_pubsub_subscription_enable_message_ordering">
    <rdfs:label>enable_message_ordering</rdfs:label>
    <rdfs:comment>If 'true', messages published with the same orderingKey in PubsubMessage will be delivered to
the subscribers in the order in which they are received by the Pub/Sub system. Otherwise, they
may be delivered in any order.</rdfs:comment>
    <rdfs:domain rdf:resource="http://example.org/onto/class/google_pubsub_subscription"/>
    <rdfs:range rdf:resource="http://www.w3.org/2001/XMLSchema#string"/>
  </owl:DatatypeProperty>
  <owl:DatatypeProperty rdf:about="http://example.org/onto/prop/google_pubsub_subscription_filter">
    <rdfs:label>filter</rdfs:label>
    <rdfs:comment>The subscription only delivers the messages that match the filter.
Pub/Sub automatically acknowledges the messages that don't match the filter. You can filter messages
by their attributes. The maximum length of a filter is 256 bytes. After creating the subscription,
you can't modify the filter.</rdfs:comment>
    <rdfs:domain rdf:resource="http://example.org/onto/class/google_pubsub_subscription"/>
    <rdfs:range rdf:resource="http://www.w3.org/2001/XMLSchema#string"/>
  </owl:DatatypeProperty>
  <owl:DatatypeProperty rdf:about="http://example.org/onto/prop/google_pubsub_subscription_id">
    <rdfs:label>id</rdfs:label>
    <rdfs:domain rdf:resource="http://example.org/onto/class/google_pubsub_subscription"/>
    <rdfs:range rdf:resource="http://www.w3.org/2001/XMLSchema#string"/>
  </owl:DatatypeProperty>
  <owl:DatatypeProperty rdf:about="http://example.org/onto/prop/google_pubsub_subscription_labels">
    <rdfs:label>labels</rdfs:label>
    <rdfs:comment>A set of key/value label pairs to assign to this Subscription.


**Note**: This field is non-authoritative, and will only manage the labels present in your configuration.
Please refer to the field 'effective_labels' for all of the labels present on the resource.</rdfs:comment>
    <rdfs:domain rdf:resource="http://example.org/onto/class/google_pubsub_subscription"/>
    <rdfs:range rdf:resource="http://www.w3.org/2001/XMLSchema#string"/>
  </owl:DatatypeProperty>
  <owl:DatatypeProperty rdf:about="http://example.org/onto/prop/google_pubsub_subscription_message_retention_duration">
    <rdfs:label>message_retention_duration</rdfs:label>
    <rdfs:comment>How long to retain unacknowledged messages in the subscription's
backlog, from the moment a message is published. If
retain_acked_messages is true, then this also configures the retention
of acknowledged messages, and thus configures how far back in time a
subscriptions.seek can be done. Defaults to 7 days. Cannot be more
than 31 days ('"2678400s"') or less than 10 minutes ('"600s"').

A duration in seconds with up to nine fractional digits, terminated
by 's'. Example: '"600.5s"'.</rdfs:comment>
    <rdfs:domain rdf:resource="http://example.org/onto/class/google_pubsub_subscription"/>
    <rdfs:range rdf:resource="http://www.w3.org/2001/XMLSchema#string"/>
  </owl:DatatypeProperty>
  <owl:DatatypeProperty rdf:about="http://example.org/onto/prop/google_pubsub_subscription_name">
    <rdfs:label>name</rdfs:label>
    <rdfs:comment>Name of the subscription.</rdfs:comment>
    <rdfs:domain rdf:resource="http://example.org/onto/class/google_pubsub_subscription"/>
    <rdfs:range rdf:resource="http://www.w3.org/2001/XMLSchema#string"/>
  </owl:DatatypeProperty>
  <owl:DatatypeProperty rdf:about="http://example.org/onto/prop/google_pubsub_subscription_project">
    <rdfs:label>project</rdfs:label>
    <rdfs:domain rdf:resource="http://example.org/onto/class/google_pubsub_subscription"/>
    <rdfs:range rdf:resource="http://www.w3.org/2001/XMLSchema#string"/>
  </owl:DatatypeProperty>
  <owl:DatatypeProperty rdf:about="http://example.org/onto/prop/google_pubsub_subscription_retain_acked_messages">
    <rdfs:label>retain_acked_messages</rdfs:label>
    <rdfs:comment>Indicates whether to retain acknowledged messages. If 'true', then
messages are not expunged from the subscription's backlog, even if
they are acknowledged, until they fall out of the
messageRetentionDuration window.</rdfs:comment>
    <rdfs:domain rdf:resource="http://example.org/onto/class/google_pubsub_subscription"/>
    <rdfs:range rdf:resource="http://www.w3.org/2001/XMLSchema#string"/>
  </owl:DatatypeProperty>
  <owl:DatatypeProperty rdf:about="http://example.org/onto/prop/google_pubsub_subscription_tags">
    <rdfs:label>tags</rdfs:label>
    <rdfs:comment>Input only. Resource manager tags to be bound to the subscription. Tag
keys and values have the same definition as resource manager tags. Keys
must be in the format tagKeys/{tag_key_id}, and values are in the format
tagValues/456. The field is ignored when empty. The field is immutable and
causes resource replacement when mutated. This field is only set at create
time and modifying this field after creation will trigger recreation. To
apply tags to an existing resource, see the 'google_tags_tag_value'
resource.</rdfs:comment>
    <rdfs:domain rdf:resource="http://example.org/onto/class/google_pubsub_subscription"/>
    <rdfs:range rdf:resource="http://www.w3.org/2001/XMLSchema#string"/>
  </owl:DatatypeProperty>
  <owl:DatatypeProperty rdf:about="http://example.org/onto/prop/google_pubsub_subscription_terraform_labels">
    <rdfs:label>terraform_labels</rdfs:label>
    <rdfs:comment>The combination of labels configured directly on the resource
 and default labels configured on the provider.</rdfs:comment>
    <rdfs:domain rdf:resource="http://example.org/onto/class/google_pubsub_subscription"/>
    <rdfs:range rdf:resource="http://www.w3.org/2001/XMLSchema#string"/>
  </owl:DatatypeProperty>
  <owl:DatatypeProperty rdf:about="http://example.org/onto/prop/google_pubsub_subscription_topic">
    <rdfs:label>topic</rdfs:label>
    <rdfs:comment>A reference to a Topic resource, of the form projects/{project}/topics/{{name}}
(as in the id property of a google_pubsub_topic), or just a topic name if
the topic is in the same project as the subscription.</rdfs:comment>
    <rdfs:domain rdf:resource="http://example.org/onto/class/google_pubsub_subscription"/>
    <rdfs:range rdf:resource="http://www.w3.org/2001/XMLSchema#string"/>
  </owl:DatatypeProperty>
  <owl:DatatypeProperty rdf:about="http://example.org/onto/prop/google_pubsub_subscription_drop_unknown_fields">
    <rdfs:label>drop_unknown_fields</rdfs:label>
    <rdfs:comment>When true and use_topic_schema or use_table_schema is true, any fields that are a part of the topic schema or message schema that
are not part of the BigQuery table schema are dropped when writing to BigQuery. Otherwise, the schemas must be kept in sync
and any messages with extra fields are not written and remain in the subscription's backlog.</rdfs:comment>
    <rdfs:domain rdf:resource="http://example.org/onto/class/google_pubsub_subscription"/>
    <rdfs:range rdf:resource="http://www.w3.org/2001/XMLSchema#string"/>
  </owl:DatatypeProperty>
  <owl:DatatypeProperty rdf:about="http://example.org/onto/prop/google_pubsub_subscription_service_account_email">
    <rdfs:label>service_account_email</rdfs:label>
    <rdfs:comment>The service account to use to write to BigQuery. If not specified, the Pub/Sub
[service agent](https://cloud.google.com/iam/docs/service-agents),
service-{project_number}@gcp-sa-pubsub.iam.gserviceaccount.com, is used.</rdfs:comment>
    <rdfs:domain rdf:resource="http://example.org/onto/class/google_pubsub_subscription"/>
    <rdfs:range rdf:resource="http://www.w3.org/2001/XMLSchema#string"/>
  </owl:DatatypeProperty>
  <owl:DatatypeProperty rdf:about="http://example.org/onto/prop/google_pubsub_subscription_table">
    <rdfs:label>table</rdfs:label>
    <rdfs:comment>The name of the table to which to write data, of the form {projectId}.{datasetId}.{tableId}</rdfs:comment>
    <rdfs:domain rdf:resource="http://example.org/onto/class/google_pubsub_subscription"/>
    <rdfs:range rdf:resource="http://www.w3.org/2001/XMLSchema#string"/>
  </owl:DatatypeProperty>
  <owl:DatatypeProperty rdf:about="http://example.org/onto/prop/google_pubsub_subscription_use_table_schema">
    <rdfs:label>use_table_schema</rdfs:label>
    <rdfs:comment>When true, use the BigQuery table's schema as the columns to write to in BigQuery. Messages
must be published in JSON format. Only one of use_topic_schema and use_table_schema can be set.</rdfs:comment>
    <rdfs:domain rdf:resource="http://example.org/onto/class/google_pubsub_subscription"/>
    <rdfs:range rdf:resource="http://www.w3.org/2001/XMLSchema#string"/>
  </owl:DatatypeProperty>
  <owl:DatatypeProperty rdf:about="http://example.org/onto/prop/google_pubsub_subscription_use_topic_schema">
    <rdfs:label>use_topic_schema</rdfs:label>
    <rdfs:comment>When true, use the topic's schema as the columns to write to in BigQuery, if it exists.
Only one of use_topic_schema and use_table_schema can be set.</rdfs:comment>
    <rdfs:domain rdf:resource="http://example.org/onto/class/google_pubsub_subscription"/>
    <rdfs:range rdf:resource="http://www.w3.org/2001/XMLSchema#string"/>
  </owl:DatatypeProperty>
  <owl:DatatypeProperty rdf:about="http://example.org/onto/prop/google_pubsub_subscription_write_metadata">
    <rdfs:label>write_metadata</rdfs:label>
    <rdfs:comment>When true, write the subscription name, messageId, publishTime, attributes, and orderingKey to additional columns in the table.
The subscription name, messageId, and publishTime fields are put in their own columns while all other message properties (other than data) are written to a JSON object in the attributes column.</rdfs:comment>
    <rdfs:domain rdf:resource="http://example.org/onto/class/google_pubsub_subscription"/>
    <rdfs:range rdf:resource="http://www.w3.org/2001/XMLSchema#string"/>
  </owl:DatatypeProperty>
  <owl:DatatypeProperty rdf:about="http://example.org/onto/prop/google_pubsub_subscription_bucket">
    <rdfs:label>bucket</rdfs:label>
    <rdfs:comment>User-provided name for the Cloud Storage bucket. The bucket must be created by the user. The bucket name must be without any prefix like "gs://".</rdfs:comment>
    <rdfs:domain rdf:resource="http://example.org/onto/class/google_pubsub_subscription"/>
    <rdfs:range rdf:resource="http://www.w3.org/2001/XMLSchema#string"/>
  </owl:DatatypeProperty>
  <owl:DatatypeProperty rdf:about="http://example.org/onto/prop/google_pubsub_subscription_filename_datetime_format">
    <rdfs:label>filename_datetime_format</rdfs:label>
    <rdfs:comment>User-provided format string specifying how to represent datetimes in Cloud Storage filenames.</rdfs:comment>
    <rdfs:domain rdf:resource="http://example.org/onto/class/google_pubsub_subscription"/>
    <rdfs:range rdf:resource="http://www.w3.org/2001/XMLSchema#string"/>
  </owl:DatatypeProperty>
  <owl:DatatypeProperty rdf:about="http://example.org/onto/prop/google_pubsub_subscription_filename_prefix">
    <rdfs:label>filename_prefix</rdfs:label>
    <rdfs:comment>User-provided prefix for Cloud Storage filename.</rdfs:comment>
    <rdfs:domain rdf:resource="http://example.org/onto/class/google_pubsub_subscription"/>
    <rdfs:range rdf:resource="http://www.w3.org/2001/XMLSchema#string"/>
  </owl:DatatypeProperty>
  <owl:DatatypeProperty rdf:about="http://example.org/onto/prop/google_pubsub_subscription_filename_suffix">
    <rdfs:label>filename_suffix</rdfs:label>
    <rdfs:comment>User-provided suffix for Cloud Storage filename. Must not end in "/".</rdfs:comment>
    <rdfs:domain rdf:resource="http://example.org/onto/class/google_pubsub_subscription"/>
    <rdfs:range rdf:resource="http://www.w3.org/2001/XMLSchema#string"/>
  </owl:DatatypeProperty>
  <owl:DatatypeProperty rdf:about="http://example.org/onto/prop/google_pubsub_subscription_max_bytes">
    <rdfs:label>max_bytes</rdfs:label>
    <rdfs:comment>The maximum bytes that can be written to a Cloud Storage file before a new file is created. Min 1 KB, max 10 GiB.
The maxBytes limit may be exceeded in cases where messages are larger than the limit.</rdfs:comment>
    <rdfs:domain rdf:resource="http://example.org/onto/class/google_pubsub_subscription"/>
    <rdfs:range rdf:resource="http://www.w3.org/2001/XMLSchema#string"/>
  </owl:DatatypeProperty>
  <owl:DatatypeProperty rdf:about="http://example.org/onto/prop/google_pubsub_subscription_max_duration">
    <rdfs:label>max_duration</rdfs:label>
    <rdfs:comment>The maximum duration that can elapse before a new Cloud Storage file is created. Min 1 minute, max 10 minutes, default 5 minutes.
May not exceed the subscription's acknowledgement deadline.
A duration in seconds with up to nine fractional digits, ending with 's'. Example: "3.5s".</rdfs:comment>
    <rdfs:domain rdf:resource="http://example.org/onto/class/google_pubsub_subscription"/>
    <rdfs:range rdf:resource="http://www.w3.org/2001/XMLSchema#string"/>
  </owl:DatatypeProperty>
  <owl:DatatypeProperty rdf:about="http://example.org/onto/prop/google_pubsub_subscription_max_messages">
    <rdfs:label>max_messages</rdfs:label>
    <rdfs:comment>The maximum messages that can be written to a Cloud Storage file before a new file is created. Min 1000 messages.</rdfs:comment>
    <rdfs:domain rdf:resource="http://example.org/onto/class/google_pubsub_subscription"/>
    <rdfs:range rdf:resource="http://www.w3.org/2001/XMLSchema#string"/>
  </owl:DatatypeProperty>
  <owl:DatatypeProperty rdf:about="http://example.org/onto/prop/google_pubsub_subscription_service_account_email">
    <rdfs:label>service_account_email</rdfs:label>
    <rdfs:comment>The service account to use to write to Cloud Storage. If not specified, the Pub/Sub
[service agent](https://cloud.google.com/iam/docs/service-agents),
service-{project_number}@gcp-sa-pubsub.iam.gserviceaccount.com, is used.</rdfs:comment>
    <rdfs:domain rdf:resource="http://example.org/onto/class/google_pubsub_subscription"/>
    <rdfs:range rdf:resource="http://www.w3.org/2001/XMLSchema#string"/>
  </owl:DatatypeProperty>
  <owl:DatatypeProperty rdf:about="http://example.org/onto/prop/google_pubsub_subscription_state">
    <rdfs:label>state</rdfs:label>
    <rdfs:comment>An output-only field that indicates whether or not the subscription can receive messages.</rdfs:comment>
    <rdfs:domain rdf:resource="http://example.org/onto/class/google_pubsub_subscription"/>
    <rdfs:range rdf:resource="http://www.w3.org/2001/XMLSchema#string"/>
  </owl:DatatypeProperty>
  <owl:DatatypeProperty rdf:about="http://example.org/onto/prop/google_pubsub_subscription_use_topic_schema">
    <rdfs:label>use_topic_schema</rdfs:label>
    <rdfs:comment>When true, the output Cloud Storage file will be serialized using the topic schema, if it exists.</rdfs:comment>
    <rdfs:domain rdf:resource="http://example.org/onto/class/google_pubsub_subscription"/>
    <rdfs:range rdf:resource="http://www.w3.org/2001/XMLSchema#string"/>
  </owl:DatatypeProperty>
  <owl:DatatypeProperty rdf:about="http://example.org/onto/prop/google_pubsub_subscription_write_metadata">
    <rdfs:label>write_metadata</rdfs:label>
    <rdfs:comment>When true, write the subscription name, messageId, publishTime, attributes, and orderingKey as additional fields in the output.</rdfs:comment>
    <rdfs:domain rdf:resource="http://example.org/onto/class/google_pubsub_subscription"/>
    <rdfs:range rdf:resource="http://www.w3.org/2001/XMLSchema#string"/>
  </owl:DatatypeProperty>
  <owl:DatatypeProperty rdf:about="http://example.org/onto/prop/google_pubsub_subscription_dead_letter_topic">
    <rdfs:label>dead_letter_topic</rdfs:label>
    <rdfs:comment>The name of the topic to which dead letter messages should be published.
Format is 'projects/{project}/topics/{topic}'.

The Cloud Pub/Sub service account associated with the enclosing subscription's
parent project (i.e.,
service-{project_number}@gcp-sa-pubsub.iam.gserviceaccount.com) must have
permission to Publish() to this topic.

The operation will fail if the topic does not exist.
Users should ensure that there is a subscription attached to this topic
since messages published to a topic with no subscriptions are lost.</rdfs:comment>
    <rdfs:domain rdf:resource="http://example.org/onto/class/google_pubsub_subscription"/>
    <rdfs:range rdf:resource="http://www.w3.org/2001/XMLSchema#string"/>
  </owl:DatatypeProperty>
  <owl:DatatypeProperty rdf:about="http://example.org/onto/prop/google_pubsub_subscription_max_delivery_attempts">
    <rdfs:label>max_delivery_attempts</rdfs:label>
    <rdfs:comment>The maximum number of delivery attempts for any message. The value must be
between 5 and 100.

The number of delivery attempts is defined as 1 + (the sum of number of
NACKs and number of times the acknowledgement deadline has been exceeded for the message).

A NACK is any call to ModifyAckDeadline with a 0 deadline. Note that
client libraries may automatically extend ack_deadlines.

This field will be honored on a best effort basis.

If this parameter is 0, a default value of 5 is used.</rdfs:comment>
    <rdfs:domain rdf:resource="http://example.org/onto/class/google_pubsub_subscription"/>
    <rdfs:range rdf:resource="http://www.w3.org/2001/XMLSchema#string"/>
  </owl:DatatypeProperty>
  <owl:DatatypeProperty rdf:about="http://example.org/onto/prop/google_pubsub_subscription_ttl">
    <rdfs:label>ttl</rdfs:label>
    <rdfs:comment>Specifies the "time-to-live" duration for an associated resource. The
resource expires if it is not active for a period of ttl.
If ttl is set to "", the associated resource never expires.
A duration in seconds with up to nine fractional digits, terminated by 's'.
Example - "3.5s".</rdfs:comment>
    <rdfs:domain rdf:resource="http://example.org/onto/class/google_pubsub_subscription"/>
    <rdfs:range rdf:resource="http://www.w3.org/2001/XMLSchema#string"/>
  </owl:DatatypeProperty>
  <owl:DatatypeProperty rdf:about="http://example.org/onto/prop/google_pubsub_subscription_disabled">
    <rdfs:label>disabled</rdfs:label>
    <rdfs:comment>Controls whether or not to use this transform. If not set or 'false',
the transform will be applied to messages. Default: 'true'.</rdfs:comment>
    <rdfs:domain rdf:resource="http://example.org/onto/class/google_pubsub_subscription"/>
    <rdfs:range rdf:resource="http://www.w3.org/2001/XMLSchema#string"/>
  </owl:DatatypeProperty>
  <owl:DatatypeProperty rdf:about="http://example.org/onto/prop/google_pubsub_subscription_code">
    <rdfs:label>code</rdfs:label>
    <rdfs:comment>JavaScript code that contains a function 'function_name' with the
following signature:
'''
  /**
  * Transforms a Pub/Sub message.
  *
  * @return {(Object<string, (string | Object<string, string>)>|null)} - To
  * filter a message, return 'null'. To transform a message return a map
  * with the following keys:
  *   - (required) 'data' : {string}
  *   - (optional) 'attributes' : {Object<string, string>}
  * Returning empty 'attributes' will remove all attributes from the
  * message.
  *
  * @param  {(Object<string, (string | Object<string, string>)>} Pub/Sub
  * message. Keys:
  *   - (required) 'data' : {string}
  *   - (required) 'attributes' : {Object<string, string>}
  *
  * @param  {Object<string, any>} metadata - Pub/Sub message metadata.
  * Keys:
  *   - (required) 'message_id'  : {string}
  *   - (optional) 'publish_time': {string} YYYY-MM-DDTHH:MM:SSZ format
  *   - (optional) 'ordering_key': {string}
  */
  function <function_name>(message, metadata) {
  }
'''</rdfs:comment>
    <rdfs:domain rdf:resource="http://example.org/onto/class/google_pubsub_subscription"/>
    <rdfs:range rdf:resource="http://www.w3.org/2001/XMLSchema#string"/>
  </owl:DatatypeProperty>
  <owl:DatatypeProperty rdf:about="http://example.org/onto/prop/google_pubsub_subscription_function_name">
    <rdfs:label>function_name</rdfs:label>
    <rdfs:comment>Name of the JavaScript function that should be applied to Pub/Sub messages.</rdfs:comment>
    <rdfs:domain rdf:resource="http://example.org/onto/class/google_pubsub_subscription"/>
    <rdfs:range rdf:resource="http://www.w3.org/2001/XMLSchema#string"/>
  </owl:DatatypeProperty>
  <owl:DatatypeProperty rdf:about="http://example.org/onto/prop/google_pubsub_subscription_attributes">
    <rdfs:label>attributes</rdfs:label>
    <rdfs:comment>Endpoint configuration attributes.

Every endpoint has a set of API supported attributes that can
be used to control different aspects of the message delivery.

The currently supported attribute is x-goog-version, which you
can use to change the format of the pushed message. This
attribute indicates the version of the data expected by
the endpoint. This controls the shape of the pushed message
(i.e., its fields and metadata). The endpoint version is
based on the version of the Pub/Sub API.

If not present during the subscriptions.create call,
it will default to the version of the API used to make
such call. If not present during a subscriptions.modifyPushConfig
call, its value will not be changed. subscriptions.get
calls will always return a valid version, even if the
subscription was created without this attribute.

The possible values for this attribute are:

- v1beta1: uses the push format defined in the v1beta1 Pub/Sub API.
- v1 or v1beta2: uses the push format defined in the v1 Pub/Sub API.</rdfs:comment>
    <rdfs:domain rdf:resource="http://example.org/onto/class/google_pubsub_subscription"/>
    <rdfs:range rdf:resource="http://www.w3.org/2001/XMLSchema#string"/>
  </owl:DatatypeProperty>
  <owl:DatatypeProperty rdf:about="http://example.org/onto/prop/google_pubsub_subscription_push_endpoint">
    <rdfs:label>push_endpoint</rdfs:label>
    <rdfs:comment>A URL locating the endpoint to which messages should be pushed.
For example, a Webhook endpoint might use
"https://example.com/push".</rdfs:comment>
    <rdfs:domain rdf:resource="http://example.org/onto/class/google_pubsub_subscription"/>
    <rdfs:range rdf:resource="http://www.w3.org/2001/XMLSchema#string"/>
  </owl:DatatypeProperty>
  <owl:DatatypeProperty rdf:about="http://example.org/onto/prop/google_pubsub_subscription_write_metadata">
    <rdfs:label>write_metadata</rdfs:label>
    <rdfs:comment>When true, writes the Pub/Sub message metadata to
'x-goog-pubsub-<KEY>:<VAL>' headers of the HTTP request. Writes the
Pub/Sub message attributes to '<KEY>:<VAL>' headers of the HTTP request.</rdfs:comment>
    <rdfs:domain rdf:resource="http://example.org/onto/class/google_pubsub_subscription"/>
    <rdfs:range rdf:resource="http://www.w3.org/2001/XMLSchema#string"/>
  </owl:DatatypeProperty>
  <owl:DatatypeProperty rdf:about="http://example.org/onto/prop/google_pubsub_subscription_audience">
    <rdfs:label>audience</rdfs:label>
    <rdfs:comment>Audience to be used when generating OIDC token. The audience claim
identifies the recipients that the JWT is intended for. The audience
value is a single case-sensitive string. Having multiple values (array)
for the audience field is not supported. More info about the OIDC JWT
token audience here: https://tools.ietf.org/html/rfc7519#section-4.1.3
Note: if not specified, the Push endpoint URL will be used.</rdfs:comment>
    <rdfs:domain rdf:resource="http://example.org/onto/class/google_pubsub_subscription"/>
    <rdfs:range rdf:resource="http://www.w3.org/2001/XMLSchema#string"/>
  </owl:DatatypeProperty>
  <owl:DatatypeProperty rdf:about="http://example.org/onto/prop/google_pubsub_subscription_service_account_email">
    <rdfs:label>service_account_email</rdfs:label>
    <rdfs:comment>Service account email to be used for generating the OIDC token.
The caller (for subscriptions.create, subscriptions.patch, and
subscriptions.modifyPushConfig RPCs) must have the
iam.serviceAccounts.actAs permission for the service account.</rdfs:comment>
    <rdfs:domain rdf:resource="http://example.org/onto/class/google_pubsub_subscription"/>
    <rdfs:range rdf:resource="http://www.w3.org/2001/XMLSchema#string"/>
  </owl:DatatypeProperty>
  <owl:DatatypeProperty rdf:about="http://example.org/onto/prop/google_pubsub_subscription_maximum_backoff">
    <rdfs:label>maximum_backoff</rdfs:label>
    <rdfs:comment>The maximum delay between consecutive deliveries of a given message. Value should be between 0 and 600 seconds. Defaults to 600 seconds.
A duration in seconds with up to nine fractional digits, terminated by 's'. Example: "3.5s".</rdfs:comment>
    <rdfs:domain rdf:resource="http://example.org/onto/class/google_pubsub_subscription"/>
    <rdfs:range rdf:resource="http://www.w3.org/2001/XMLSchema#string"/>
  </owl:DatatypeProperty>
  <owl:DatatypeProperty rdf:about="http://example.org/onto/prop/google_pubsub_subscription_minimum_backoff">
    <rdfs:label>minimum_backoff</rdfs:label>
    <rdfs:comment>The minimum delay between consecutive deliveries of a given message. Value should be between 0 and 600 seconds. Defaults to 10 seconds.
A duration in seconds with up to nine fractional digits, terminated by 's'. Example: "3.5s".</rdfs:comment>
    <rdfs:domain rdf:resource="http://example.org/onto/class/google_pubsub_subscription"/>
    <rdfs:range rdf:resource="http://www.w3.org/2001/XMLSchema#string"/>
  </owl:DatatypeProperty>
  <owl:DatatypeProperty rdf:about="http://example.org/onto/prop/google_pubsub_subscription_create">
    <rdfs:label>create</rdfs:label>
    <rdfs:domain rdf:resource="http://example.org/onto/class/google_pubsub_subscription"/>
    <rdfs:range rdf:resource="http://www.w3.org/2001/XMLSchema#string"/>
  </owl:DatatypeProperty>
  <owl:DatatypeProperty rdf:about="http://example.org/onto/prop/google_pubsub_subscription_delete">
    <rdfs:label>delete</rdfs:label>
    <rdfs:domain rdf:resource="http://example.org/onto/class/google_pubsub_subscription"/>
    <rdfs:range rdf:resource="http://www.w3.org/2001/XMLSchema#string"/>
  </owl:DatatypeProperty>
  <owl:DatatypeProperty rdf:about="http://example.org/onto/prop/google_pubsub_subscription_update">
    <rdfs:label>update</rdfs:label>
    <rdfs:domain rdf:resource="http://example.org/onto/class/google_pubsub_subscription"/>
    <rdfs:range rdf:resource="http://www.w3.org/2001/XMLSchema#string"/>
  </owl:DatatypeProperty>
</rdf:RDF>
