<?xml version="1.0" encoding="UTF-8"?>
<rdf:RDF
  xmlns:rdf="http://www.w3.org/1999/02/22-rdf-syntax-ns#"
  xmlns:rdfs="http://www.w3.org/2000/01/rdf-schema#"
  xmlns:owl="http://www.w3.org/2002/07/owl#"
  xmlns:xsd="http://www.w3.org/2001/XMLSchema#"
  xml:base="http://example.org/onto/">
  <owl:Class rdf:about="http://example.org/onto/class/google_compute_resize_request">
    <rdfs:label>google_compute_resize_request</rdfs:label>
    <rdfs:comment>#
#     ***     AUTO GENERATED CODE    ***    Type: MMv1     ***
#
# ----------------------------------------------------------------------------
#
#     This code is generated by Magic Modules using the following:
#
#     Configuration: https:#github.com/GoogleCloudPlatform/magic-modules/tree/main/mmv1/products/compute/ResizeRequest.yaml
#     Template:      https:#github.com/GoogleCloudPlatform/magic-modules/tree/main/mmv1/templates/terraform/resource.html.markdown.tmpl
#
#     DO NOT EDIT this file directly. Any changes made to this file will be
#     overwritten during the next generation cycle.
#
# ----------------------------------------------------------------------------
subcategory: "Compute Engine"
description: |-
  Represents a Managed Instance Group Resize Request
  Resize Requests are the Managed Instance Group implementation of Dynamic Workload Scheduler Flex Start.
---</rdfs:comment>
  </owl:Class>
  <owl:DatatypeProperty rdf:about="http://example.org/onto/prop/google_compute_resize_request_creation_timestamp">
    <rdfs:label>creation_timestamp</rdfs:label>
    <rdfs:comment>The creation timestamp for this resize request in RFC3339 text format.</rdfs:comment>
    <rdfs:domain rdf:resource="http://example.org/onto/class/google_compute_resize_request"/>
    <rdfs:range rdf:resource="http://www.w3.org/2001/XMLSchema#string"/>
  </owl:DatatypeProperty>
  <owl:DatatypeProperty rdf:about="http://example.org/onto/prop/google_compute_resize_request_description">
    <rdfs:label>description</rdfs:label>
    <rdfs:comment>An optional description of this resize-request.</rdfs:comment>
    <rdfs:domain rdf:resource="http://example.org/onto/class/google_compute_resize_request"/>
    <rdfs:range rdf:resource="http://www.w3.org/2001/XMLSchema#string"/>
  </owl:DatatypeProperty>
  <owl:DatatypeProperty rdf:about="http://example.org/onto/prop/google_compute_resize_request_id">
    <rdfs:label>id</rdfs:label>
    <rdfs:domain rdf:resource="http://example.org/onto/class/google_compute_resize_request"/>
    <rdfs:range rdf:resource="http://www.w3.org/2001/XMLSchema#string"/>
  </owl:DatatypeProperty>
  <owl:DatatypeProperty rdf:about="http://example.org/onto/prop/google_compute_resize_request_instance_group_manager">
    <rdfs:label>instance_group_manager</rdfs:label>
    <rdfs:comment>The reference of the instance group manager this ResizeRequest is a part of.</rdfs:comment>
    <rdfs:domain rdf:resource="http://example.org/onto/class/google_compute_resize_request"/>
    <rdfs:range rdf:resource="http://www.w3.org/2001/XMLSchema#string"/>
  </owl:DatatypeProperty>
  <owl:DatatypeProperty rdf:about="http://example.org/onto/prop/google_compute_resize_request_name">
    <rdfs:label>name</rdfs:label>
    <rdfs:comment>The name of this resize request. The name must be 1-63 characters long, and comply with RFC1035.</rdfs:comment>
    <rdfs:domain rdf:resource="http://example.org/onto/class/google_compute_resize_request"/>
    <rdfs:range rdf:resource="http://www.w3.org/2001/XMLSchema#string"/>
  </owl:DatatypeProperty>
  <owl:DatatypeProperty rdf:about="http://example.org/onto/prop/google_compute_resize_request_project">
    <rdfs:label>project</rdfs:label>
    <rdfs:domain rdf:resource="http://example.org/onto/class/google_compute_resize_request"/>
    <rdfs:range rdf:resource="http://www.w3.org/2001/XMLSchema#string"/>
  </owl:DatatypeProperty>
  <owl:DatatypeProperty rdf:about="http://example.org/onto/prop/google_compute_resize_request_resize_by">
    <rdfs:label>resize_by</rdfs:label>
    <rdfs:comment>The number of instances to be created by this resize request. The group's target size will be increased by this number.</rdfs:comment>
    <rdfs:domain rdf:resource="http://example.org/onto/class/google_compute_resize_request"/>
    <rdfs:range rdf:resource="http://www.w3.org/2001/XMLSchema#string"/>
  </owl:DatatypeProperty>
  <owl:DatatypeProperty rdf:about="http://example.org/onto/prop/google_compute_resize_request_state">
    <rdfs:label>state</rdfs:label>
    <rdfs:comment>Current state of the request.</rdfs:comment>
    <rdfs:domain rdf:resource="http://example.org/onto/class/google_compute_resize_request"/>
    <rdfs:range rdf:resource="http://www.w3.org/2001/XMLSchema#string"/>
  </owl:DatatypeProperty>
  <owl:DatatypeProperty rdf:about="http://example.org/onto/prop/google_compute_resize_request_status">
    <rdfs:label>status</rdfs:label>
    <rdfs:comment>Status of the request.</rdfs:comment>
    <rdfs:domain rdf:resource="http://example.org/onto/class/google_compute_resize_request"/>
    <rdfs:range rdf:resource="http://www.w3.org/2001/XMLSchema#string"/>
  </owl:DatatypeProperty>
  <owl:DatatypeProperty rdf:about="http://example.org/onto/prop/google_compute_resize_request_zone">
    <rdfs:label>zone</rdfs:label>
    <rdfs:comment>The reference of the compute zone scoping this request. If it is not provided, the provider zone is used.</rdfs:comment>
    <rdfs:domain rdf:resource="http://example.org/onto/class/google_compute_resize_request"/>
    <rdfs:range rdf:resource="http://www.w3.org/2001/XMLSchema#string"/>
  </owl:DatatypeProperty>
  <owl:DatatypeProperty rdf:about="http://example.org/onto/prop/google_compute_resize_request_nanos">
    <rdfs:label>nanos</rdfs:label>
    <rdfs:comment>Span of time that's a fraction of a second at nanosecond resolution. Durations less than one second are represented with a 0 seconds field and a positive nanos field. Must be from 0 to 999,999,999 inclusive.</rdfs:comment>
    <rdfs:domain rdf:resource="http://example.org/onto/class/google_compute_resize_request"/>
    <rdfs:range rdf:resource="http://www.w3.org/2001/XMLSchema#string"/>
  </owl:DatatypeProperty>
  <owl:DatatypeProperty rdf:about="http://example.org/onto/prop/google_compute_resize_request_seconds">
    <rdfs:label>seconds</rdfs:label>
    <rdfs:comment>Span of time at a resolution of a second. Must be from 600 to 604800 inclusive. Note: minimum and maximum allowed range for requestedRunDuration is 10 minutes (600 seconds) and 7 days(604800 seconds) correspondingly.</rdfs:comment>
    <rdfs:domain rdf:resource="http://example.org/onto/class/google_compute_resize_request"/>
    <rdfs:range rdf:resource="http://www.w3.org/2001/XMLSchema#string"/>
  </owl:DatatypeProperty>
  <owl:DatatypeProperty rdf:about="http://example.org/onto/prop/google_compute_resize_request_create">
    <rdfs:label>create</rdfs:label>
    <rdfs:domain rdf:resource="http://example.org/onto/class/google_compute_resize_request"/>
    <rdfs:range rdf:resource="http://www.w3.org/2001/XMLSchema#string"/>
  </owl:DatatypeProperty>
  <owl:DatatypeProperty rdf:about="http://example.org/onto/prop/google_compute_resize_request_delete">
    <rdfs:label>delete</rdfs:label>
    <rdfs:domain rdf:resource="http://example.org/onto/class/google_compute_resize_request"/>
    <rdfs:range rdf:resource="http://www.w3.org/2001/XMLSchema#string"/>
  </owl:DatatypeProperty>
</rdf:RDF>
