<?xml version="1.0" encoding="UTF-8"?>
<rdf:RDF
  xmlns:rdf="http://www.w3.org/1999/02/22-rdf-syntax-ns#"
  xmlns:rdfs="http://www.w3.org/2000/01/rdf-schema#"
  xmlns:owl="http://www.w3.org/2002/07/owl#"
  xmlns:xsd="http://www.w3.org/2001/XMLSchema#"
  xml:base="http://example.org/onto/">
  <owl:Class rdf:about="http://example.org/onto/class/google_chronicle_rule_deployment">
    <rdfs:label>google_chronicle_rule_deployment</rdfs:label>
    <rdfs:comment>#
#     ***     AUTO GENERATED CODE    ***    Type: MMv1     ***
#
# ----------------------------------------------------------------------------
#
#     This code is generated by Magic Modules using the following:
#
#     Configuration: https:#github.com/GoogleCloudPlatform/magic-modules/tree/main/mmv1/products/chronicle/RuleDeployment.yaml
#     Template:      https:#github.com/GoogleCloudPlatform/magic-modules/tree/main/mmv1/templates/terraform/resource.html.markdown.tmpl
#
#     DO NOT EDIT this file directly. Any changes made to this file will be
#     overwritten during the next generation cycle.
#
# ----------------------------------------------------------------------------
subcategory: "Chronicle"
description: |-
  The RuleDeployment resource represents the deployment state of a Rule.
---</rdfs:comment>
  </owl:Class>
  <owl:DatatypeProperty rdf:about="http://example.org/onto/prop/google_chronicle_rule_deployment_alerting">
    <rdfs:label>alerting</rdfs:label>
    <rdfs:comment>Whether detections resulting from this deployment should be considered
alerts.</rdfs:comment>
    <rdfs:domain rdf:resource="http://example.org/onto/class/google_chronicle_rule_deployment"/>
    <rdfs:range rdf:resource="http://www.w3.org/2001/XMLSchema#string"/>
  </owl:DatatypeProperty>
  <owl:DatatypeProperty rdf:about="http://example.org/onto/prop/google_chronicle_rule_deployment_archive_time">
    <rdfs:label>archive_time</rdfs:label>
    <rdfs:comment>Output only. The timestamp when the rule deployment archive state was last set to true. If the rule deployment's current archive state is not set to true, the field will be empty.</rdfs:comment>
    <rdfs:domain rdf:resource="http://example.org/onto/class/google_chronicle_rule_deployment"/>
    <rdfs:range rdf:resource="http://www.w3.org/2001/XMLSchema#string"/>
  </owl:DatatypeProperty>
  <owl:DatatypeProperty rdf:about="http://example.org/onto/prop/google_chronicle_rule_deployment_archived">
    <rdfs:label>archived</rdfs:label>
    <rdfs:comment>The archive state of the rule deployment.
Cannot be set to true unless enabled is set to false i.e.
archiving requires a two-step process: first, disable the rule by
setting 'enabled' to false, then set 'archive' to true.
If set to true, alerting will automatically be set to false.
If currently set to true, enabled, alerting, and run_frequency cannot be
updated.</rdfs:comment>
    <rdfs:domain rdf:resource="http://example.org/onto/class/google_chronicle_rule_deployment"/>
    <rdfs:range rdf:resource="http://www.w3.org/2001/XMLSchema#string"/>
  </owl:DatatypeProperty>
  <owl:DatatypeProperty rdf:about="http://example.org/onto/prop/google_chronicle_rule_deployment_consumer_rules">
    <rdfs:label>consumer_rules</rdfs:label>
    <rdfs:comment>Output only. The names of the associated/chained consumer rules. Rules are considered
consumers of this rule if their rule text explicitly filters on this rule's ruleid.
Format:
projects/{project}/locations/{location}/instances/{instance}/rules/{rule}</rdfs:comment>
    <rdfs:domain rdf:resource="http://example.org/onto/class/google_chronicle_rule_deployment"/>
    <rdfs:range rdf:resource="http://www.w3.org/2001/XMLSchema#string"/>
  </owl:DatatypeProperty>
  <owl:DatatypeProperty rdf:about="http://example.org/onto/prop/google_chronicle_rule_deployment_enabled">
    <rdfs:label>enabled</rdfs:label>
    <rdfs:comment>Whether the rule is currently deployed continuously against incoming data.</rdfs:comment>
    <rdfs:domain rdf:resource="http://example.org/onto/class/google_chronicle_rule_deployment"/>
    <rdfs:range rdf:resource="http://www.w3.org/2001/XMLSchema#string"/>
  </owl:DatatypeProperty>
  <owl:DatatypeProperty rdf:about="http://example.org/onto/prop/google_chronicle_rule_deployment_execution_state">
    <rdfs:label>execution_state</rdfs:label>
    <rdfs:comment>The execution state of the rule deployment.
Possible values:
DEFAULT
LIMITED
PAUSED</rdfs:comment>
    <rdfs:domain rdf:resource="http://example.org/onto/class/google_chronicle_rule_deployment"/>
    <rdfs:range rdf:resource="http://www.w3.org/2001/XMLSchema#string"/>
  </owl:DatatypeProperty>
  <owl:DatatypeProperty rdf:about="http://example.org/onto/prop/google_chronicle_rule_deployment_id">
    <rdfs:label>id</rdfs:label>
    <rdfs:domain rdf:resource="http://example.org/onto/class/google_chronicle_rule_deployment"/>
    <rdfs:range rdf:resource="http://www.w3.org/2001/XMLSchema#string"/>
  </owl:DatatypeProperty>
  <owl:DatatypeProperty rdf:about="http://example.org/onto/prop/google_chronicle_rule_deployment_instance">
    <rdfs:label>instance</rdfs:label>
    <rdfs:comment>The unique identifier for the Chronicle instance, which is the same as the customer ID.</rdfs:comment>
    <rdfs:domain rdf:resource="http://example.org/onto/class/google_chronicle_rule_deployment"/>
    <rdfs:range rdf:resource="http://www.w3.org/2001/XMLSchema#string"/>
  </owl:DatatypeProperty>
  <owl:DatatypeProperty rdf:about="http://example.org/onto/prop/google_chronicle_rule_deployment_last_alert_status_change_time">
    <rdfs:label>last_alert_status_change_time</rdfs:label>
    <rdfs:comment>Output only. The timestamp when the rule deployment alert state was lastly changed. This is filled regardless of the current alert state.E.g. if the current alert status is false, this timestamp will be the timestamp when the alert status was changed to false.</rdfs:comment>
    <rdfs:domain rdf:resource="http://example.org/onto/class/google_chronicle_rule_deployment"/>
    <rdfs:range rdf:resource="http://www.w3.org/2001/XMLSchema#string"/>
  </owl:DatatypeProperty>
  <owl:DatatypeProperty rdf:about="http://example.org/onto/prop/google_chronicle_rule_deployment_location">
    <rdfs:label>location</rdfs:label>
    <rdfs:comment>The location of the resource. This is the geographical region where the Chronicle instance resides, such as "us" or "europe-west2".</rdfs:comment>
    <rdfs:domain rdf:resource="http://example.org/onto/class/google_chronicle_rule_deployment"/>
    <rdfs:range rdf:resource="http://www.w3.org/2001/XMLSchema#string"/>
  </owl:DatatypeProperty>
  <owl:DatatypeProperty rdf:about="http://example.org/onto/prop/google_chronicle_rule_deployment_name">
    <rdfs:label>name</rdfs:label>
    <rdfs:comment>The resource name of the rule deployment.
Note that RuleDeployment is a child of the overall Rule, not any individual
revision, so the resource ID segment for the Rule resource must not
reference a specific revision.
Format:
projects/{project}/locations/{location}/instances/{instance}/rules/{rule}/deployment</rdfs:comment>
    <rdfs:domain rdf:resource="http://example.org/onto/class/google_chronicle_rule_deployment"/>
    <rdfs:range rdf:resource="http://www.w3.org/2001/XMLSchema#string"/>
  </owl:DatatypeProperty>
  <owl:DatatypeProperty rdf:about="http://example.org/onto/prop/google_chronicle_rule_deployment_producer_rules">
    <rdfs:label>producer_rules</rdfs:label>
    <rdfs:comment>Output only. The names of the associated/chained producer rules. Rules are considered
producers for this rule if this rule explicitly filters on their ruleid.
Format:
projects/{project}/locations/{location}/instances/{instance}/rules/{rule}</rdfs:comment>
    <rdfs:domain rdf:resource="http://example.org/onto/class/google_chronicle_rule_deployment"/>
    <rdfs:range rdf:resource="http://www.w3.org/2001/XMLSchema#string"/>
  </owl:DatatypeProperty>
  <owl:DatatypeProperty rdf:about="http://example.org/onto/prop/google_chronicle_rule_deployment_project">
    <rdfs:label>project</rdfs:label>
    <rdfs:domain rdf:resource="http://example.org/onto/class/google_chronicle_rule_deployment"/>
    <rdfs:range rdf:resource="http://www.w3.org/2001/XMLSchema#string"/>
  </owl:DatatypeProperty>
  <owl:DatatypeProperty rdf:about="http://example.org/onto/prop/google_chronicle_rule_deployment_rule">
    <rdfs:label>rule</rdfs:label>
    <rdfs:comment>The Rule ID of the rule.</rdfs:comment>
    <rdfs:domain rdf:resource="http://example.org/onto/class/google_chronicle_rule_deployment"/>
    <rdfs:range rdf:resource="http://www.w3.org/2001/XMLSchema#string"/>
  </owl:DatatypeProperty>
  <owl:DatatypeProperty rdf:about="http://example.org/onto/prop/google_chronicle_rule_deployment_run_frequency">
    <rdfs:label>run_frequency</rdfs:label>
    <rdfs:comment>The run frequency of the rule deployment.
Possible values:
LIVE
HOURLY
DAILY</rdfs:comment>
    <rdfs:domain rdf:resource="http://example.org/onto/class/google_chronicle_rule_deployment"/>
    <rdfs:range rdf:resource="http://www.w3.org/2001/XMLSchema#string"/>
  </owl:DatatypeProperty>
  <owl:DatatypeProperty rdf:about="http://example.org/onto/prop/google_chronicle_rule_deployment_create">
    <rdfs:label>create</rdfs:label>
    <rdfs:domain rdf:resource="http://example.org/onto/class/google_chronicle_rule_deployment"/>
    <rdfs:range rdf:resource="http://www.w3.org/2001/XMLSchema#string"/>
  </owl:DatatypeProperty>
  <owl:DatatypeProperty rdf:about="http://example.org/onto/prop/google_chronicle_rule_deployment_delete">
    <rdfs:label>delete</rdfs:label>
    <rdfs:domain rdf:resource="http://example.org/onto/class/google_chronicle_rule_deployment"/>
    <rdfs:range rdf:resource="http://www.w3.org/2001/XMLSchema#string"/>
  </owl:DatatypeProperty>
  <owl:DatatypeProperty rdf:about="http://example.org/onto/prop/google_chronicle_rule_deployment_update">
    <rdfs:label>update</rdfs:label>
    <rdfs:domain rdf:resource="http://example.org/onto/class/google_chronicle_rule_deployment"/>
    <rdfs:range rdf:resource="http://www.w3.org/2001/XMLSchema#string"/>
  </owl:DatatypeProperty>
</rdf:RDF>
