<?xml version="1.0" encoding="UTF-8"?>
<rdf:RDF
  xmlns:rdf="http://www.w3.org/1999/02/22-rdf-syntax-ns#"
  xmlns:rdfs="http://www.w3.org/2000/01/rdf-schema#"
  xmlns:owl="http://www.w3.org/2002/07/owl#"
  xmlns:xsd="http://www.w3.org/2001/XMLSchema#"
  xml:base="http://example.org/onto/">
  <owl:Class rdf:about="http://example.org/onto/class/google_active_directory_domain_trust">
    <rdfs:label>google_active_directory_domain_trust</rdfs:label>
    <rdfs:comment>#
#     ***     AUTO GENERATED CODE    ***    Type: MMv1     ***
#
# ----------------------------------------------------------------------------
#
#     This code is generated by Magic Modules using the following:
#
#     Configuration: https:#github.com/GoogleCloudPlatform/magic-modules/tree/main/mmv1/products/activedirectory/DomainTrust.yaml
#     Template:      https:#github.com/GoogleCloudPlatform/magic-modules/tree/main/mmv1/templates/terraform/resource.html.markdown.tmpl
#
#     DO NOT EDIT this file directly. Any changes made to this file will be
#     overwritten during the next generation cycle.
#
# ----------------------------------------------------------------------------
subcategory: "Managed Microsoft Active Directory"
description: |-
  Adds a trust between Active Directory domains
---</rdfs:comment>
  </owl:Class>
  <owl:DatatypeProperty rdf:about="http://example.org/onto/prop/google_active_directory_domain_trust_domain">
    <rdfs:label>domain</rdfs:label>
    <rdfs:comment>The fully qualified domain name. e.g. mydomain.myorganization.com, with the restrictions
of https://cloud.google.com/managed-microsoft-ad/reference/rest/v1/projects.locations.global.domains.</rdfs:comment>
    <rdfs:domain rdf:resource="http://example.org/onto/class/google_active_directory_domain_trust"/>
    <rdfs:range rdf:resource="http://www.w3.org/2001/XMLSchema#string"/>
  </owl:DatatypeProperty>
  <owl:DatatypeProperty rdf:about="http://example.org/onto/prop/google_active_directory_domain_trust_id">
    <rdfs:label>id</rdfs:label>
    <rdfs:domain rdf:resource="http://example.org/onto/class/google_active_directory_domain_trust"/>
    <rdfs:range rdf:resource="http://www.w3.org/2001/XMLSchema#string"/>
  </owl:DatatypeProperty>
  <owl:DatatypeProperty rdf:about="http://example.org/onto/prop/google_active_directory_domain_trust_project">
    <rdfs:label>project</rdfs:label>
    <rdfs:domain rdf:resource="http://example.org/onto/class/google_active_directory_domain_trust"/>
    <rdfs:range rdf:resource="http://www.w3.org/2001/XMLSchema#string"/>
  </owl:DatatypeProperty>
  <owl:DatatypeProperty rdf:about="http://example.org/onto/prop/google_active_directory_domain_trust_selective_authentication">
    <rdfs:label>selective_authentication</rdfs:label>
    <rdfs:comment>Whether the trusted side has forest/domain wide access or selective access to an approved set of resources.</rdfs:comment>
    <rdfs:domain rdf:resource="http://example.org/onto/class/google_active_directory_domain_trust"/>
    <rdfs:range rdf:resource="http://www.w3.org/2001/XMLSchema#string"/>
  </owl:DatatypeProperty>
  <owl:DatatypeProperty rdf:about="http://example.org/onto/prop/google_active_directory_domain_trust_target_dns_ip_addresses">
    <rdfs:label>target_dns_ip_addresses</rdfs:label>
    <rdfs:comment>The target DNS server IP addresses which can resolve the remote domain involved in the trust.</rdfs:comment>
    <rdfs:domain rdf:resource="http://example.org/onto/class/google_active_directory_domain_trust"/>
    <rdfs:range rdf:resource="http://www.w3.org/2001/XMLSchema#string"/>
  </owl:DatatypeProperty>
  <owl:DatatypeProperty rdf:about="http://example.org/onto/prop/google_active_directory_domain_trust_target_domain_name">
    <rdfs:label>target_domain_name</rdfs:label>
    <rdfs:comment>The fully qualified target domain name which will be in trust with the current domain.</rdfs:comment>
    <rdfs:domain rdf:resource="http://example.org/onto/class/google_active_directory_domain_trust"/>
    <rdfs:range rdf:resource="http://www.w3.org/2001/XMLSchema#string"/>
  </owl:DatatypeProperty>
  <owl:DatatypeProperty rdf:about="http://example.org/onto/prop/google_active_directory_domain_trust_trust_direction">
    <rdfs:label>trust_direction</rdfs:label>
    <rdfs:comment>The trust direction, which decides if the current domain is trusted, trusting, or both. Possible values: ["INBOUND", "OUTBOUND", "BIDIRECTIONAL"]</rdfs:comment>
    <rdfs:domain rdf:resource="http://example.org/onto/class/google_active_directory_domain_trust"/>
    <rdfs:range rdf:resource="http://www.w3.org/2001/XMLSchema#string"/>
  </owl:DatatypeProperty>
  <owl:DatatypeProperty rdf:about="http://example.org/onto/prop/google_active_directory_domain_trust_trust_handshake_secret">
    <rdfs:label>trust_handshake_secret</rdfs:label>
    <rdfs:comment>The trust secret used for the handshake with the target domain. This will not be stored.</rdfs:comment>
    <rdfs:domain rdf:resource="http://example.org/onto/class/google_active_directory_domain_trust"/>
    <rdfs:range rdf:resource="http://www.w3.org/2001/XMLSchema#string"/>
  </owl:DatatypeProperty>
  <owl:DatatypeProperty rdf:about="http://example.org/onto/prop/google_active_directory_domain_trust_trust_type">
    <rdfs:label>trust_type</rdfs:label>
    <rdfs:comment>The type of trust represented by the trust resource. Possible values: ["FOREST", "EXTERNAL"]</rdfs:comment>
    <rdfs:domain rdf:resource="http://example.org/onto/class/google_active_directory_domain_trust"/>
    <rdfs:range rdf:resource="http://www.w3.org/2001/XMLSchema#string"/>
  </owl:DatatypeProperty>
  <owl:DatatypeProperty rdf:about="http://example.org/onto/prop/google_active_directory_domain_trust_create">
    <rdfs:label>create</rdfs:label>
    <rdfs:domain rdf:resource="http://example.org/onto/class/google_active_directory_domain_trust"/>
    <rdfs:range rdf:resource="http://www.w3.org/2001/XMLSchema#string"/>
  </owl:DatatypeProperty>
  <owl:DatatypeProperty rdf:about="http://example.org/onto/prop/google_active_directory_domain_trust_delete">
    <rdfs:label>delete</rdfs:label>
    <rdfs:domain rdf:resource="http://example.org/onto/class/google_active_directory_domain_trust"/>
    <rdfs:range rdf:resource="http://www.w3.org/2001/XMLSchema#string"/>
  </owl:DatatypeProperty>
  <owl:DatatypeProperty rdf:about="http://example.org/onto/prop/google_active_directory_domain_trust_update">
    <rdfs:label>update</rdfs:label>
    <rdfs:domain rdf:resource="http://example.org/onto/class/google_active_directory_domain_trust"/>
    <rdfs:range rdf:resource="http://www.w3.org/2001/XMLSchema#string"/>
  </owl:DatatypeProperty>
</rdf:RDF>
