<?xml version="1.0" encoding="UTF-8"?>
<rdf:RDF
  xmlns:rdf="http://www.w3.org/1999/02/22-rdf-syntax-ns#"
  xmlns:rdfs="http://www.w3.org/2000/01/rdf-schema#"
  xmlns:owl="http://www.w3.org/2002/07/owl#"
  xmlns:xsd="http://www.w3.org/2001/XMLSchema#"
  xml:base="http://example.org/onto/">
  <owl:Class rdf:about="http://example.org/onto/class/google_org_policy_policy">
    <rdfs:label>google_org_policy_policy</rdfs:label>
    <rdfs:comment>#
#     ***     AUTO GENERATED CODE    ***    Type: MMv1     ***
#
# ----------------------------------------------------------------------------
#
#     This code is generated by Magic Modules using the following:
#
#     Configuration: https:#github.com/GoogleCloudPlatform/magic-modules/tree/main/mmv1/products/orgpolicy/Policy.yaml
#     Template:      https:#github.com/GoogleCloudPlatform/magic-modules/tree/main/mmv1/templates/terraform/resource.html.markdown.tmpl
#
#     DO NOT EDIT this file directly. Any changes made to this file will be
#     overwritten during the next generation cycle.
#
# ----------------------------------------------------------------------------
subcategory: "Organization Policy"
description: |-
  Defines an organization policy which is used to specify constraints for configurations of Google Cloud resources.
---</rdfs:comment>
  </owl:Class>
  <owl:DatatypeProperty rdf:about="http://example.org/onto/prop/google_org_policy_policy_etag">
    <rdfs:label>etag</rdfs:label>
    <rdfs:comment>Optional. An opaque tag indicating the current state of the policy, used for concurrency control. This 'etag' is computed by the server based on the value of other fields, and may be sent on update and delete requests to ensure the client has an up-to-date value before proceeding.</rdfs:comment>
    <rdfs:domain rdf:resource="http://example.org/onto/class/google_org_policy_policy"/>
    <rdfs:range rdf:resource="http://www.w3.org/2001/XMLSchema#string"/>
  </owl:DatatypeProperty>
  <owl:DatatypeProperty rdf:about="http://example.org/onto/prop/google_org_policy_policy_id">
    <rdfs:label>id</rdfs:label>
    <rdfs:domain rdf:resource="http://example.org/onto/class/google_org_policy_policy"/>
    <rdfs:range rdf:resource="http://www.w3.org/2001/XMLSchema#string"/>
  </owl:DatatypeProperty>
  <owl:DatatypeProperty rdf:about="http://example.org/onto/prop/google_org_policy_policy_name">
    <rdfs:label>name</rdfs:label>
    <rdfs:comment>Immutable. The resource name of the Policy. Must be one of the following forms, where constraint_name is the name of the constraint which this Policy configures: * 'projects/{project_number}/policies/{constraint_name}' * 'folders/{folder_id}/policies/{constraint_name}' * 'organizations/{organization_id}/policies/{constraint_name}' For example, "projects/123/policies/compute.disableSerialPortAccess". Note: 'projects/{project_id}/policies/{constraint_name}' is also an acceptable name for API requests, but responses will return the name using the equivalent project number.</rdfs:comment>
    <rdfs:domain rdf:resource="http://example.org/onto/class/google_org_policy_policy"/>
    <rdfs:range rdf:resource="http://www.w3.org/2001/XMLSchema#string"/>
  </owl:DatatypeProperty>
  <owl:DatatypeProperty rdf:about="http://example.org/onto/prop/google_org_policy_policy_parent">
    <rdfs:label>parent</rdfs:label>
    <rdfs:comment>The parent of the resource.</rdfs:comment>
    <rdfs:domain rdf:resource="http://example.org/onto/class/google_org_policy_policy"/>
    <rdfs:range rdf:resource="http://www.w3.org/2001/XMLSchema#string"/>
  </owl:DatatypeProperty>
  <owl:DatatypeProperty rdf:about="http://example.org/onto/prop/google_org_policy_policy_etag">
    <rdfs:label>etag</rdfs:label>
    <rdfs:comment>An opaque tag indicating the current version of the policy, used for concurrency control. This field is ignored if used in a 'CreatePolicy' request. When the policy' is returned from either a 'GetPolicy' or a 'ListPolicies' request, this 'etag' indicates the version of the current policy to use when executing a read-modify-write loop. When the policy is returned from a 'GetEffectivePolicy' request, the 'etag' will be unset.</rdfs:comment>
    <rdfs:domain rdf:resource="http://example.org/onto/class/google_org_policy_policy"/>
    <rdfs:range rdf:resource="http://www.w3.org/2001/XMLSchema#string"/>
  </owl:DatatypeProperty>
  <owl:DatatypeProperty rdf:about="http://example.org/onto/prop/google_org_policy_policy_inherit_from_parent">
    <rdfs:label>inherit_from_parent</rdfs:label>
    <rdfs:comment>Determines the inheritance behavior for this policy. If 'inherit_from_parent' is true, policy rules set higher up in the hierarchy (up to the closest root) are inherited and present in the effective policy. If it is false, then no rules are inherited, and this policy becomes the new root for evaluation. This field can be set only for policies which configure list constraints.</rdfs:comment>
    <rdfs:domain rdf:resource="http://example.org/onto/class/google_org_policy_policy"/>
    <rdfs:range rdf:resource="http://www.w3.org/2001/XMLSchema#string"/>
  </owl:DatatypeProperty>
  <owl:DatatypeProperty rdf:about="http://example.org/onto/prop/google_org_policy_policy_reset">
    <rdfs:label>reset</rdfs:label>
    <rdfs:comment>Ignores policies set above this resource and restores the 'constraint_default' enforcement behavior of the specific constraint at this resource. This field can be set in policies for either list or boolean constraints. If set, 'rules' must be empty and 'inherit_from_parent' must be set to false.</rdfs:comment>
    <rdfs:domain rdf:resource="http://example.org/onto/class/google_org_policy_policy"/>
    <rdfs:range rdf:resource="http://www.w3.org/2001/XMLSchema#string"/>
  </owl:DatatypeProperty>
  <owl:DatatypeProperty rdf:about="http://example.org/onto/prop/google_org_policy_policy_update_time">
    <rdfs:label>update_time</rdfs:label>
    <rdfs:comment>Output only. The time stamp this was previously updated. This represents the last time a call to 'CreatePolicy' or 'UpdatePolicy' was made for that policy.</rdfs:comment>
    <rdfs:domain rdf:resource="http://example.org/onto/class/google_org_policy_policy"/>
    <rdfs:range rdf:resource="http://www.w3.org/2001/XMLSchema#string"/>
  </owl:DatatypeProperty>
  <owl:DatatypeProperty rdf:about="http://example.org/onto/prop/google_org_policy_policy_allow_all">
    <rdfs:label>allow_all</rdfs:label>
    <rdfs:comment>Setting this to '"TRUE"' means that all values are allowed. This field can be set only in Policies for list constraints.</rdfs:comment>
    <rdfs:domain rdf:resource="http://example.org/onto/class/google_org_policy_policy"/>
    <rdfs:range rdf:resource="http://www.w3.org/2001/XMLSchema#string"/>
  </owl:DatatypeProperty>
  <owl:DatatypeProperty rdf:about="http://example.org/onto/prop/google_org_policy_policy_deny_all">
    <rdfs:label>deny_all</rdfs:label>
    <rdfs:comment>Setting this to '"TRUE"' means that all values are denied. This field can be set only in Policies for list constraints.</rdfs:comment>
    <rdfs:domain rdf:resource="http://example.org/onto/class/google_org_policy_policy"/>
    <rdfs:range rdf:resource="http://www.w3.org/2001/XMLSchema#string"/>
  </owl:DatatypeProperty>
  <owl:DatatypeProperty rdf:about="http://example.org/onto/prop/google_org_policy_policy_enforce">
    <rdfs:label>enforce</rdfs:label>
    <rdfs:comment>If '"TRUE"', then the 'Policy' is enforced. If '"FALSE"', then any configuration is acceptable. This field can be set only in Policies for boolean constraints.</rdfs:comment>
    <rdfs:domain rdf:resource="http://example.org/onto/class/google_org_policy_policy"/>
    <rdfs:range rdf:resource="http://www.w3.org/2001/XMLSchema#string"/>
  </owl:DatatypeProperty>
  <owl:DatatypeProperty rdf:about="http://example.org/onto/prop/google_org_policy_policy_parameters">
    <rdfs:label>parameters</rdfs:label>
    <rdfs:comment>Optional. Required for Managed Constraints if parameters defined in constraints. Pass parameter values when policy enforcement is enabled. Ensure that parameter value types match those defined in the constraint definition. For example: { \"allowedLocations\" : [\"us-east1\", \"us-west1\"], \"allowAll\" : true }</rdfs:comment>
    <rdfs:domain rdf:resource="http://example.org/onto/class/google_org_policy_policy"/>
    <rdfs:range rdf:resource="http://www.w3.org/2001/XMLSchema#string"/>
  </owl:DatatypeProperty>
  <owl:DatatypeProperty rdf:about="http://example.org/onto/prop/google_org_policy_policy_description">
    <rdfs:label>description</rdfs:label>
    <rdfs:comment>Optional. Description of the expression. This is a longer text which describes the expression, e.g. when hovered over it in a UI.</rdfs:comment>
    <rdfs:domain rdf:resource="http://example.org/onto/class/google_org_policy_policy"/>
    <rdfs:range rdf:resource="http://www.w3.org/2001/XMLSchema#string"/>
  </owl:DatatypeProperty>
  <owl:DatatypeProperty rdf:about="http://example.org/onto/prop/google_org_policy_policy_expression">
    <rdfs:label>expression</rdfs:label>
    <rdfs:comment>Textual representation of an expression in Common Expression Language syntax.</rdfs:comment>
    <rdfs:domain rdf:resource="http://example.org/onto/class/google_org_policy_policy"/>
    <rdfs:range rdf:resource="http://www.w3.org/2001/XMLSchema#string"/>
  </owl:DatatypeProperty>
  <owl:DatatypeProperty rdf:about="http://example.org/onto/prop/google_org_policy_policy_location">
    <rdfs:label>location</rdfs:label>
    <rdfs:comment>Optional. String indicating the location of the expression for error reporting, e.g. a file name and a position in the file.</rdfs:comment>
    <rdfs:domain rdf:resource="http://example.org/onto/class/google_org_policy_policy"/>
    <rdfs:range rdf:resource="http://www.w3.org/2001/XMLSchema#string"/>
  </owl:DatatypeProperty>
  <owl:DatatypeProperty rdf:about="http://example.org/onto/prop/google_org_policy_policy_title">
    <rdfs:label>title</rdfs:label>
    <rdfs:comment>Optional. Title for the expression, i.e. a short string describing its purpose. This can be used e.g. in UIs which allow to enter the expression.</rdfs:comment>
    <rdfs:domain rdf:resource="http://example.org/onto/class/google_org_policy_policy"/>
    <rdfs:range rdf:resource="http://www.w3.org/2001/XMLSchema#string"/>
  </owl:DatatypeProperty>
  <owl:DatatypeProperty rdf:about="http://example.org/onto/prop/google_org_policy_policy_allowed_values">
    <rdfs:label>allowed_values</rdfs:label>
    <rdfs:comment>List of values allowed at this resource.</rdfs:comment>
    <rdfs:domain rdf:resource="http://example.org/onto/class/google_org_policy_policy"/>
    <rdfs:range rdf:resource="http://www.w3.org/2001/XMLSchema#string"/>
  </owl:DatatypeProperty>
  <owl:DatatypeProperty rdf:about="http://example.org/onto/prop/google_org_policy_policy_denied_values">
    <rdfs:label>denied_values</rdfs:label>
    <rdfs:comment>List of values denied at this resource.</rdfs:comment>
    <rdfs:domain rdf:resource="http://example.org/onto/class/google_org_policy_policy"/>
    <rdfs:range rdf:resource="http://www.w3.org/2001/XMLSchema#string"/>
  </owl:DatatypeProperty>
  <owl:DatatypeProperty rdf:about="http://example.org/onto/prop/google_org_policy_policy_etag">
    <rdfs:label>etag</rdfs:label>
    <rdfs:comment>An opaque tag indicating the current version of the 'Policy', used for concurrency control. This field is ignored if used in a 'CreatePolicy' request. When the 'Policy' is returned from either a 'GetPolicy' or a 'ListPolicies' request, this 'etag' indicates the version of the current 'Policy' to use when executing a read-modify-write loop. When the 'Policy' is returned from a 'GetEffectivePolicy' request, the 'etag' will be unset.</rdfs:comment>
    <rdfs:domain rdf:resource="http://example.org/onto/class/google_org_policy_policy"/>
    <rdfs:range rdf:resource="http://www.w3.org/2001/XMLSchema#string"/>
  </owl:DatatypeProperty>
  <owl:DatatypeProperty rdf:about="http://example.org/onto/prop/google_org_policy_policy_inherit_from_parent">
    <rdfs:label>inherit_from_parent</rdfs:label>
    <rdfs:comment>Determines the inheritance behavior for this 'Policy'. If 'inherit_from_parent' is true, PolicyRules set higher up in the hierarchy (up to the closest root) are inherited and present in the effective policy. If it is false, then no rules are inherited, and this Policy becomes the new root for evaluation. This field can be set only for Policies which configure list constraints.</rdfs:comment>
    <rdfs:domain rdf:resource="http://example.org/onto/class/google_org_policy_policy"/>
    <rdfs:range rdf:resource="http://www.w3.org/2001/XMLSchema#string"/>
  </owl:DatatypeProperty>
  <owl:DatatypeProperty rdf:about="http://example.org/onto/prop/google_org_policy_policy_reset">
    <rdfs:label>reset</rdfs:label>
    <rdfs:comment>Ignores policies set above this resource and restores the 'constraint_default' enforcement behavior of the specific 'Constraint' at this resource. This field can be set in policies for either list or boolean constraints. If set, 'rules' must be empty and 'inherit_from_parent' must be set to false.</rdfs:comment>
    <rdfs:domain rdf:resource="http://example.org/onto/class/google_org_policy_policy"/>
    <rdfs:range rdf:resource="http://www.w3.org/2001/XMLSchema#string"/>
  </owl:DatatypeProperty>
  <owl:DatatypeProperty rdf:about="http://example.org/onto/prop/google_org_policy_policy_update_time">
    <rdfs:label>update_time</rdfs:label>
    <rdfs:comment>Output only. The time stamp this was previously updated. This represents the last time a call to 'CreatePolicy' or 'UpdatePolicy' was made for that 'Policy'.</rdfs:comment>
    <rdfs:domain rdf:resource="http://example.org/onto/class/google_org_policy_policy"/>
    <rdfs:range rdf:resource="http://www.w3.org/2001/XMLSchema#string"/>
  </owl:DatatypeProperty>
  <owl:DatatypeProperty rdf:about="http://example.org/onto/prop/google_org_policy_policy_allow_all">
    <rdfs:label>allow_all</rdfs:label>
    <rdfs:comment>Setting this to '"TRUE"' means that all values are allowed. This field can be set only in Policies for list constraints.</rdfs:comment>
    <rdfs:domain rdf:resource="http://example.org/onto/class/google_org_policy_policy"/>
    <rdfs:range rdf:resource="http://www.w3.org/2001/XMLSchema#string"/>
  </owl:DatatypeProperty>
  <owl:DatatypeProperty rdf:about="http://example.org/onto/prop/google_org_policy_policy_deny_all">
    <rdfs:label>deny_all</rdfs:label>
    <rdfs:comment>Setting this to '"TRUE"' means that all values are denied. This field can be set only in Policies for list constraints.</rdfs:comment>
    <rdfs:domain rdf:resource="http://example.org/onto/class/google_org_policy_policy"/>
    <rdfs:range rdf:resource="http://www.w3.org/2001/XMLSchema#string"/>
  </owl:DatatypeProperty>
  <owl:DatatypeProperty rdf:about="http://example.org/onto/prop/google_org_policy_policy_enforce">
    <rdfs:label>enforce</rdfs:label>
    <rdfs:comment>If '"TRUE"', then the 'Policy' is enforced. If '"FALSE"', then any configuration is acceptable. This field can be set only in Policies for boolean constraints.</rdfs:comment>
    <rdfs:domain rdf:resource="http://example.org/onto/class/google_org_policy_policy"/>
    <rdfs:range rdf:resource="http://www.w3.org/2001/XMLSchema#string"/>
  </owl:DatatypeProperty>
  <owl:DatatypeProperty rdf:about="http://example.org/onto/prop/google_org_policy_policy_parameters">
    <rdfs:label>parameters</rdfs:label>
    <rdfs:comment>Optional. Required for Managed Constraints if parameters defined in constraints. Pass parameter values when policy enforcement is enabled. Ensure that parameter value types match those defined in the constraint definition. For example: { \"allowedLocations\" : [\"us-east1\", \"us-west1\"], \"allowAll\" : true }</rdfs:comment>
    <rdfs:domain rdf:resource="http://example.org/onto/class/google_org_policy_policy"/>
    <rdfs:range rdf:resource="http://www.w3.org/2001/XMLSchema#string"/>
  </owl:DatatypeProperty>
  <owl:DatatypeProperty rdf:about="http://example.org/onto/prop/google_org_policy_policy_description">
    <rdfs:label>description</rdfs:label>
    <rdfs:comment>Optional. Description of the expression. This is a longer text which describes the expression, e.g. when hovered over it in a UI.</rdfs:comment>
    <rdfs:domain rdf:resource="http://example.org/onto/class/google_org_policy_policy"/>
    <rdfs:range rdf:resource="http://www.w3.org/2001/XMLSchema#string"/>
  </owl:DatatypeProperty>
  <owl:DatatypeProperty rdf:about="http://example.org/onto/prop/google_org_policy_policy_expression">
    <rdfs:label>expression</rdfs:label>
    <rdfs:comment>Textual representation of an expression in Common Expression Language syntax.</rdfs:comment>
    <rdfs:domain rdf:resource="http://example.org/onto/class/google_org_policy_policy"/>
    <rdfs:range rdf:resource="http://www.w3.org/2001/XMLSchema#string"/>
  </owl:DatatypeProperty>
  <owl:DatatypeProperty rdf:about="http://example.org/onto/prop/google_org_policy_policy_location">
    <rdfs:label>location</rdfs:label>
    <rdfs:comment>Optional. String indicating the location of the expression for error reporting, e.g. a file name and a position in the file.</rdfs:comment>
    <rdfs:domain rdf:resource="http://example.org/onto/class/google_org_policy_policy"/>
    <rdfs:range rdf:resource="http://www.w3.org/2001/XMLSchema#string"/>
  </owl:DatatypeProperty>
  <owl:DatatypeProperty rdf:about="http://example.org/onto/prop/google_org_policy_policy_title">
    <rdfs:label>title</rdfs:label>
    <rdfs:comment>Optional. Title for the expression, i.e. a short string describing its purpose. This can be used e.g. in UIs which allow to enter the expression.</rdfs:comment>
    <rdfs:domain rdf:resource="http://example.org/onto/class/google_org_policy_policy"/>
    <rdfs:range rdf:resource="http://www.w3.org/2001/XMLSchema#string"/>
  </owl:DatatypeProperty>
  <owl:DatatypeProperty rdf:about="http://example.org/onto/prop/google_org_policy_policy_allowed_values">
    <rdfs:label>allowed_values</rdfs:label>
    <rdfs:comment>List of values allowed at this resource.</rdfs:comment>
    <rdfs:domain rdf:resource="http://example.org/onto/class/google_org_policy_policy"/>
    <rdfs:range rdf:resource="http://www.w3.org/2001/XMLSchema#string"/>
  </owl:DatatypeProperty>
  <owl:DatatypeProperty rdf:about="http://example.org/onto/prop/google_org_policy_policy_denied_values">
    <rdfs:label>denied_values</rdfs:label>
    <rdfs:comment>List of values denied at this resource.</rdfs:comment>
    <rdfs:domain rdf:resource="http://example.org/onto/class/google_org_policy_policy"/>
    <rdfs:range rdf:resource="http://www.w3.org/2001/XMLSchema#string"/>
  </owl:DatatypeProperty>
  <owl:DatatypeProperty rdf:about="http://example.org/onto/prop/google_org_policy_policy_create">
    <rdfs:label>create</rdfs:label>
    <rdfs:domain rdf:resource="http://example.org/onto/class/google_org_policy_policy"/>
    <rdfs:range rdf:resource="http://www.w3.org/2001/XMLSchema#string"/>
  </owl:DatatypeProperty>
  <owl:DatatypeProperty rdf:about="http://example.org/onto/prop/google_org_policy_policy_delete">
    <rdfs:label>delete</rdfs:label>
    <rdfs:domain rdf:resource="http://example.org/onto/class/google_org_policy_policy"/>
    <rdfs:range rdf:resource="http://www.w3.org/2001/XMLSchema#string"/>
  </owl:DatatypeProperty>
  <owl:DatatypeProperty rdf:about="http://example.org/onto/prop/google_org_policy_policy_update">
    <rdfs:label>update</rdfs:label>
    <rdfs:domain rdf:resource="http://example.org/onto/class/google_org_policy_policy"/>
    <rdfs:range rdf:resource="http://www.w3.org/2001/XMLSchema#string"/>
  </owl:DatatypeProperty>
</rdf:RDF>
