<?xml version="1.0" encoding="UTF-8"?>
<rdf:RDF
  xmlns:rdf="http://www.w3.org/1999/02/22-rdf-syntax-ns#"
  xmlns:rdfs="http://www.w3.org/2000/01/rdf-schema#"
  xmlns:owl="http://www.w3.org/2002/07/owl#"
  xmlns:xsd="http://www.w3.org/2001/XMLSchema#"
  xml:base="http://example.org/onto/">
  <owl:Class rdf:about="http://example.org/onto/class/google_developer_connect_git_repository_link">
    <rdfs:label>google_developer_connect_git_repository_link</rdfs:label>
    <rdfs:comment>#
#     ***     AUTO GENERATED CODE    ***    Type: MMv1     ***
#
# ----------------------------------------------------------------------------
#
#     This code is generated by Magic Modules using the following:
#
#     Configuration: https:#github.com/GoogleCloudPlatform/magic-modules/tree/main/mmv1/products/developerconnect/GitRepositoryLink.yaml
#     Template:      https:#github.com/GoogleCloudPlatform/magic-modules/tree/main/mmv1/templates/terraform/resource.html.markdown.tmpl
#
#     DO NOT EDIT this file directly. Any changes made to this file will be
#     overwritten during the next generation cycle.
#
# ----------------------------------------------------------------------------
subcategory: "Developer Connect"
description: |-
  A git repository link to a parent connection.
---</rdfs:comment>
  </owl:Class>
  <owl:DatatypeProperty rdf:about="http://example.org/onto/prop/google_developer_connect_git_repository_link_annotations">
    <rdfs:label>annotations</rdfs:label>
    <rdfs:comment>Optional. Allows clients to store small amounts of arbitrary data. 

**Note**: This field is non-authoritative, and will only manage the annotations present in your configuration.
Please refer to the field 'effective_annotations' for all of the annotations present on the resource.</rdfs:comment>
    <rdfs:domain rdf:resource="http://example.org/onto/class/google_developer_connect_git_repository_link"/>
    <rdfs:range rdf:resource="http://www.w3.org/2001/XMLSchema#string"/>
  </owl:DatatypeProperty>
  <owl:DatatypeProperty rdf:about="http://example.org/onto/prop/google_developer_connect_git_repository_link_clone_uri">
    <rdfs:label>clone_uri</rdfs:label>
    <rdfs:comment>Required. Git Clone URI.</rdfs:comment>
    <rdfs:domain rdf:resource="http://example.org/onto/class/google_developer_connect_git_repository_link"/>
    <rdfs:range rdf:resource="http://www.w3.org/2001/XMLSchema#string"/>
  </owl:DatatypeProperty>
  <owl:DatatypeProperty rdf:about="http://example.org/onto/prop/google_developer_connect_git_repository_link_create_time">
    <rdfs:label>create_time</rdfs:label>
    <rdfs:comment>Output only. [Output only] Create timestamp</rdfs:comment>
    <rdfs:domain rdf:resource="http://example.org/onto/class/google_developer_connect_git_repository_link"/>
    <rdfs:range rdf:resource="http://www.w3.org/2001/XMLSchema#string"/>
  </owl:DatatypeProperty>
  <owl:DatatypeProperty rdf:about="http://example.org/onto/prop/google_developer_connect_git_repository_link_delete_time">
    <rdfs:label>delete_time</rdfs:label>
    <rdfs:comment>Output only. [Output only] Delete timestamp</rdfs:comment>
    <rdfs:domain rdf:resource="http://example.org/onto/class/google_developer_connect_git_repository_link"/>
    <rdfs:range rdf:resource="http://www.w3.org/2001/XMLSchema#string"/>
  </owl:DatatypeProperty>
  <owl:DatatypeProperty rdf:about="http://example.org/onto/prop/google_developer_connect_git_repository_link_effective_annotations">
    <rdfs:label>effective_annotations</rdfs:label>
    <rdfs:comment>All of annotations (key/value pairs) present on the resource in GCP, including the annotations configured through Terraform, other clients and services.</rdfs:comment>
    <rdfs:domain rdf:resource="http://example.org/onto/class/google_developer_connect_git_repository_link"/>
    <rdfs:range rdf:resource="http://www.w3.org/2001/XMLSchema#string"/>
  </owl:DatatypeProperty>
  <owl:DatatypeProperty rdf:about="http://example.org/onto/prop/google_developer_connect_git_repository_link_effective_labels">
    <rdfs:label>effective_labels</rdfs:label>
    <rdfs:comment>All of labels (key/value pairs) present on the resource in GCP, including the labels configured through Terraform, other clients and services.</rdfs:comment>
    <rdfs:domain rdf:resource="http://example.org/onto/class/google_developer_connect_git_repository_link"/>
    <rdfs:range rdf:resource="http://www.w3.org/2001/XMLSchema#string"/>
  </owl:DatatypeProperty>
  <owl:DatatypeProperty rdf:about="http://example.org/onto/prop/google_developer_connect_git_repository_link_etag">
    <rdfs:label>etag</rdfs:label>
    <rdfs:comment>Optional. This checksum is computed by the server based on the value of other
fields, and may be sent on update and delete requests to ensure the
client has an up-to-date value before proceeding.</rdfs:comment>
    <rdfs:domain rdf:resource="http://example.org/onto/class/google_developer_connect_git_repository_link"/>
    <rdfs:range rdf:resource="http://www.w3.org/2001/XMLSchema#string"/>
  </owl:DatatypeProperty>
  <owl:DatatypeProperty rdf:about="http://example.org/onto/prop/google_developer_connect_git_repository_link_git_repository_link_id">
    <rdfs:label>git_repository_link_id</rdfs:label>
    <rdfs:comment>Required. The ID to use for the repository, which will become the final component of
the repository's resource name. This ID should be unique in the connection.
Allows alphanumeric characters and any of -._~%!$&'()*+,;=@.</rdfs:comment>
    <rdfs:domain rdf:resource="http://example.org/onto/class/google_developer_connect_git_repository_link"/>
    <rdfs:range rdf:resource="http://www.w3.org/2001/XMLSchema#string"/>
  </owl:DatatypeProperty>
  <owl:DatatypeProperty rdf:about="http://example.org/onto/prop/google_developer_connect_git_repository_link_id">
    <rdfs:label>id</rdfs:label>
    <rdfs:domain rdf:resource="http://example.org/onto/class/google_developer_connect_git_repository_link"/>
    <rdfs:range rdf:resource="http://www.w3.org/2001/XMLSchema#string"/>
  </owl:DatatypeProperty>
  <owl:DatatypeProperty rdf:about="http://example.org/onto/prop/google_developer_connect_git_repository_link_labels">
    <rdfs:label>labels</rdfs:label>
    <rdfs:comment>Optional. Labels as key value pairs 

**Note**: This field is non-authoritative, and will only manage the labels present in your configuration.
Please refer to the field 'effective_labels' for all of the labels present on the resource.</rdfs:comment>
    <rdfs:domain rdf:resource="http://example.org/onto/class/google_developer_connect_git_repository_link"/>
    <rdfs:range rdf:resource="http://www.w3.org/2001/XMLSchema#string"/>
  </owl:DatatypeProperty>
  <owl:DatatypeProperty rdf:about="http://example.org/onto/prop/google_developer_connect_git_repository_link_location">
    <rdfs:label>location</rdfs:label>
    <rdfs:comment>Resource ID segment making up resource 'name'. It identifies the resource within its parent collection as described in https://google.aip.dev/122. See documentation for resource type 'developerconnect.googleapis.com/GitRepositoryLink'.</rdfs:comment>
    <rdfs:domain rdf:resource="http://example.org/onto/class/google_developer_connect_git_repository_link"/>
    <rdfs:range rdf:resource="http://www.w3.org/2001/XMLSchema#string"/>
  </owl:DatatypeProperty>
  <owl:DatatypeProperty rdf:about="http://example.org/onto/prop/google_developer_connect_git_repository_link_name">
    <rdfs:label>name</rdfs:label>
    <rdfs:comment>Identifier. Resource name of the repository, in the format
'projects/*/locations/*/connections/*/gitRepositoryLinks/*'.</rdfs:comment>
    <rdfs:domain rdf:resource="http://example.org/onto/class/google_developer_connect_git_repository_link"/>
    <rdfs:range rdf:resource="http://www.w3.org/2001/XMLSchema#string"/>
  </owl:DatatypeProperty>
  <owl:DatatypeProperty rdf:about="http://example.org/onto/prop/google_developer_connect_git_repository_link_parent_connection">
    <rdfs:label>parent_connection</rdfs:label>
    <rdfs:comment>Resource ID segment making up resource 'name'. It identifies the resource within its parent collection as described in https://google.aip.dev/122. See documentation for resource type 'developerconnect.googleapis.com/GitRepositoryLink'.</rdfs:comment>
    <rdfs:domain rdf:resource="http://example.org/onto/class/google_developer_connect_git_repository_link"/>
    <rdfs:range rdf:resource="http://www.w3.org/2001/XMLSchema#string"/>
  </owl:DatatypeProperty>
  <owl:DatatypeProperty rdf:about="http://example.org/onto/prop/google_developer_connect_git_repository_link_project">
    <rdfs:label>project</rdfs:label>
    <rdfs:domain rdf:resource="http://example.org/onto/class/google_developer_connect_git_repository_link"/>
    <rdfs:range rdf:resource="http://www.w3.org/2001/XMLSchema#string"/>
  </owl:DatatypeProperty>
  <owl:DatatypeProperty rdf:about="http://example.org/onto/prop/google_developer_connect_git_repository_link_reconciling">
    <rdfs:label>reconciling</rdfs:label>
    <rdfs:comment>Output only. Set to true when the connection is being set up or updated in the
background.</rdfs:comment>
    <rdfs:domain rdf:resource="http://example.org/onto/class/google_developer_connect_git_repository_link"/>
    <rdfs:range rdf:resource="http://www.w3.org/2001/XMLSchema#string"/>
  </owl:DatatypeProperty>
  <owl:DatatypeProperty rdf:about="http://example.org/onto/prop/google_developer_connect_git_repository_link_terraform_labels">
    <rdfs:label>terraform_labels</rdfs:label>
    <rdfs:comment>The combination of labels configured directly on the resource
 and default labels configured on the provider.</rdfs:comment>
    <rdfs:domain rdf:resource="http://example.org/onto/class/google_developer_connect_git_repository_link"/>
    <rdfs:range rdf:resource="http://www.w3.org/2001/XMLSchema#string"/>
  </owl:DatatypeProperty>
  <owl:DatatypeProperty rdf:about="http://example.org/onto/prop/google_developer_connect_git_repository_link_uid">
    <rdfs:label>uid</rdfs:label>
    <rdfs:comment>Output only. A system-assigned unique identifier for a the GitRepositoryLink.</rdfs:comment>
    <rdfs:domain rdf:resource="http://example.org/onto/class/google_developer_connect_git_repository_link"/>
    <rdfs:range rdf:resource="http://www.w3.org/2001/XMLSchema#string"/>
  </owl:DatatypeProperty>
  <owl:DatatypeProperty rdf:about="http://example.org/onto/prop/google_developer_connect_git_repository_link_update_time">
    <rdfs:label>update_time</rdfs:label>
    <rdfs:comment>Output only. [Output only] Update timestamp</rdfs:comment>
    <rdfs:domain rdf:resource="http://example.org/onto/class/google_developer_connect_git_repository_link"/>
    <rdfs:range rdf:resource="http://www.w3.org/2001/XMLSchema#string"/>
  </owl:DatatypeProperty>
  <owl:DatatypeProperty rdf:about="http://example.org/onto/prop/google_developer_connect_git_repository_link_create">
    <rdfs:label>create</rdfs:label>
    <rdfs:domain rdf:resource="http://example.org/onto/class/google_developer_connect_git_repository_link"/>
    <rdfs:range rdf:resource="http://www.w3.org/2001/XMLSchema#string"/>
  </owl:DatatypeProperty>
  <owl:DatatypeProperty rdf:about="http://example.org/onto/prop/google_developer_connect_git_repository_link_delete">
    <rdfs:label>delete</rdfs:label>
    <rdfs:domain rdf:resource="http://example.org/onto/class/google_developer_connect_git_repository_link"/>
    <rdfs:range rdf:resource="http://www.w3.org/2001/XMLSchema#string"/>
  </owl:DatatypeProperty>
  <owl:DatatypeProperty rdf:about="http://example.org/onto/prop/google_developer_connect_git_repository_link_update">
    <rdfs:label>update</rdfs:label>
    <rdfs:domain rdf:resource="http://example.org/onto/class/google_developer_connect_git_repository_link"/>
    <rdfs:range rdf:resource="http://www.w3.org/2001/XMLSchema#string"/>
  </owl:DatatypeProperty>
</rdf:RDF>
