<?xml version="1.0" encoding="UTF-8"?>
<rdf:RDF
  xmlns:rdf="http://www.w3.org/1999/02/22-rdf-syntax-ns#"
  xmlns:rdfs="http://www.w3.org/2000/01/rdf-schema#"
  xmlns:owl="http://www.w3.org/2002/07/owl#"
  xmlns:xsd="http://www.w3.org/2001/XMLSchema#"
  xml:base="http://example.org/onto/">
  <owl:Class rdf:about="http://example.org/onto/class/google_firestore_database">
    <rdfs:label>google_firestore_database</rdfs:label>
    <rdfs:comment>#
#     ***     AUTO GENERATED CODE    ***    Type: MMv1     ***
#
# ----------------------------------------------------------------------------
#
#     This code is generated by Magic Modules using the following:
#
#     Configuration: https:#github.com/GoogleCloudPlatform/magic-modules/tree/main/mmv1/products/firestore/Database.yaml
#     Template:      https:#github.com/GoogleCloudPlatform/magic-modules/tree/main/mmv1/templates/terraform/resource.html.markdown.tmpl
#
#     DO NOT EDIT this file directly. Any changes made to this file will be
#     overwritten during the next generation cycle.
#
# ----------------------------------------------------------------------------
subcategory: "Firestore"
description: |-
  A Cloud Firestore Database.
---</rdfs:comment>
  </owl:Class>
  <owl:DatatypeProperty rdf:about="http://example.org/onto/prop/google_firestore_database_app_engine_integration_mode">
    <rdfs:label>app_engine_integration_mode</rdfs:label>
    <rdfs:comment>The App Engine integration mode to use for this database. Possible values: ["ENABLED", "DISABLED"]</rdfs:comment>
    <rdfs:domain rdf:resource="http://example.org/onto/class/google_firestore_database"/>
    <rdfs:range rdf:resource="http://www.w3.org/2001/XMLSchema#string"/>
  </owl:DatatypeProperty>
  <owl:DatatypeProperty rdf:about="http://example.org/onto/prop/google_firestore_database_concurrency_mode">
    <rdfs:label>concurrency_mode</rdfs:label>
    <rdfs:comment>The concurrency control mode to use for this database. Possible values: ["OPTIMISTIC", "PESSIMISTIC", "OPTIMISTIC_WITH_ENTITY_GROUPS"]</rdfs:comment>
    <rdfs:domain rdf:resource="http://example.org/onto/class/google_firestore_database"/>
    <rdfs:range rdf:resource="http://www.w3.org/2001/XMLSchema#string"/>
  </owl:DatatypeProperty>
  <owl:DatatypeProperty rdf:about="http://example.org/onto/prop/google_firestore_database_create_time">
    <rdfs:label>create_time</rdfs:label>
    <rdfs:comment>Output only. The timestamp at which this database was created.</rdfs:comment>
    <rdfs:domain rdf:resource="http://example.org/onto/class/google_firestore_database"/>
    <rdfs:range rdf:resource="http://www.w3.org/2001/XMLSchema#string"/>
  </owl:DatatypeProperty>
  <owl:DatatypeProperty rdf:about="http://example.org/onto/prop/google_firestore_database_database_edition">
    <rdfs:label>database_edition</rdfs:label>
    <rdfs:comment>The database edition. Possible values: ["STANDARD", "ENTERPRISE"]</rdfs:comment>
    <rdfs:domain rdf:resource="http://example.org/onto/class/google_firestore_database"/>
    <rdfs:range rdf:resource="http://www.w3.org/2001/XMLSchema#string"/>
  </owl:DatatypeProperty>
  <owl:DatatypeProperty rdf:about="http://example.org/onto/prop/google_firestore_database_delete_protection_state">
    <rdfs:label>delete_protection_state</rdfs:label>
    <rdfs:comment>State of delete protection for the database.
When delete protection is enabled, this database cannot be deleted.
The default value is 'DELETE_PROTECTION_STATE_UNSPECIFIED', which is currently equivalent to 'DELETE_PROTECTION_DISABLED'.
**Note:** Additionally, to delete this database using 'terraform destroy', 'deletion_policy' must be set to 'DELETE'. Possible values: ["DELETE_PROTECTION_STATE_UNSPECIFIED", "DELETE_PROTECTION_ENABLED", "DELETE_PROTECTION_DISABLED"]</rdfs:comment>
    <rdfs:domain rdf:resource="http://example.org/onto/class/google_firestore_database"/>
    <rdfs:range rdf:resource="http://www.w3.org/2001/XMLSchema#string"/>
  </owl:DatatypeProperty>
  <owl:DatatypeProperty rdf:about="http://example.org/onto/prop/google_firestore_database_deletion_policy">
    <rdfs:label>deletion_policy</rdfs:label>
    <rdfs:comment>Deletion behavior for this database.
If the deletion policy is 'ABANDON', the database will be removed from Terraform state but not deleted from Google Cloud upon destruction.
If the deletion policy is 'DELETE', the database will both be removed from Terraform state and deleted from Google Cloud upon destruction.
The default value is 'ABANDON'.
See also 'delete_protection'.</rdfs:comment>
    <rdfs:domain rdf:resource="http://example.org/onto/class/google_firestore_database"/>
    <rdfs:range rdf:resource="http://www.w3.org/2001/XMLSchema#string"/>
  </owl:DatatypeProperty>
  <owl:DatatypeProperty rdf:about="http://example.org/onto/prop/google_firestore_database_earliest_version_time">
    <rdfs:label>earliest_version_time</rdfs:label>
    <rdfs:comment>Output only. The earliest timestamp at which older versions of the data can be read from the database. See versionRetentionPeriod above; this field is populated with now - versionRetentionPeriod.
This value is continuously updated, and becomes stale the moment it is queried. If you are using this value to recover data, make sure to account for the time from the moment when the value is queried to the moment when you initiate the recovery.
A timestamp in RFC3339 UTC "Zulu" format, with nanosecond resolution and up to nine fractional digits. Examples: "2014-10-02T15:01:23Z" and "2014-10-02T15:01:23.045123456Z".</rdfs:comment>
    <rdfs:domain rdf:resource="http://example.org/onto/class/google_firestore_database"/>
    <rdfs:range rdf:resource="http://www.w3.org/2001/XMLSchema#string"/>
  </owl:DatatypeProperty>
  <owl:DatatypeProperty rdf:about="http://example.org/onto/prop/google_firestore_database_etag">
    <rdfs:label>etag</rdfs:label>
    <rdfs:comment>Output only. This checksum is computed by the server based on the value of other fields,
and may be sent on update and delete requests to ensure the client has an
up-to-date value before proceeding.</rdfs:comment>
    <rdfs:domain rdf:resource="http://example.org/onto/class/google_firestore_database"/>
    <rdfs:range rdf:resource="http://www.w3.org/2001/XMLSchema#string"/>
  </owl:DatatypeProperty>
  <owl:DatatypeProperty rdf:about="http://example.org/onto/prop/google_firestore_database_id">
    <rdfs:label>id</rdfs:label>
    <rdfs:domain rdf:resource="http://example.org/onto/class/google_firestore_database"/>
    <rdfs:range rdf:resource="http://www.w3.org/2001/XMLSchema#string"/>
  </owl:DatatypeProperty>
  <owl:DatatypeProperty rdf:about="http://example.org/onto/prop/google_firestore_database_key_prefix">
    <rdfs:label>key_prefix</rdfs:label>
    <rdfs:comment>Output only. The keyPrefix for this database.
This keyPrefix is used, in combination with the project id ("~") to construct the application id
that is returned from the Cloud Datastore APIs in Google App Engine first generation runtimes.
This value may be empty in which case the appid to use for URL-encoded keys is the project_id (eg: foo instead of v~foo).</rdfs:comment>
    <rdfs:domain rdf:resource="http://example.org/onto/class/google_firestore_database"/>
    <rdfs:range rdf:resource="http://www.w3.org/2001/XMLSchema#string"/>
  </owl:DatatypeProperty>
  <owl:DatatypeProperty rdf:about="http://example.org/onto/prop/google_firestore_database_location_id">
    <rdfs:label>location_id</rdfs:label>
    <rdfs:comment>The location of the database. Available locations are listed at
https://cloud.google.com/firestore/docs/locations.</rdfs:comment>
    <rdfs:domain rdf:resource="http://example.org/onto/class/google_firestore_database"/>
    <rdfs:range rdf:resource="http://www.w3.org/2001/XMLSchema#string"/>
  </owl:DatatypeProperty>
  <owl:DatatypeProperty rdf:about="http://example.org/onto/prop/google_firestore_database_name">
    <rdfs:label>name</rdfs:label>
    <rdfs:comment>The ID to use for the database, which will become the final
component of the database's resource name. This value should be 4-63
characters. Valid characters are /[a-z][0-9]-/ with first character
a letter and the last a letter or a number. Must not be
UUID-like /[0-9a-f]{8}(-[0-9a-f]{4}){3}-[0-9a-f]{12}/.
"(default)" database id is also valid.</rdfs:comment>
    <rdfs:domain rdf:resource="http://example.org/onto/class/google_firestore_database"/>
    <rdfs:range rdf:resource="http://www.w3.org/2001/XMLSchema#string"/>
  </owl:DatatypeProperty>
  <owl:DatatypeProperty rdf:about="http://example.org/onto/prop/google_firestore_database_point_in_time_recovery_enablement">
    <rdfs:label>point_in_time_recovery_enablement</rdfs:label>
    <rdfs:comment>Whether to enable the PITR feature on this database.
If 'POINT_IN_TIME_RECOVERY_ENABLED' is selected, reads are supported on selected versions of the data from within the past 7 days.
versionRetentionPeriod and earliestVersionTime can be used to determine the supported versions. These include reads against any timestamp within the past hour
and reads against 1-minute snapshots beyond 1 hour and within 7 days.
If 'POINT_IN_TIME_RECOVERY_DISABLED' is selected, reads are supported on any version of the data from within the past 1 hour. Default value: "POINT_IN_TIME_RECOVERY_DISABLED" Possible values: ["POINT_IN_TIME_RECOVERY_ENABLED", "POINT_IN_TIME_RECOVERY_DISABLED"]</rdfs:comment>
    <rdfs:domain rdf:resource="http://example.org/onto/class/google_firestore_database"/>
    <rdfs:range rdf:resource="http://www.w3.org/2001/XMLSchema#string"/>
  </owl:DatatypeProperty>
  <owl:DatatypeProperty rdf:about="http://example.org/onto/prop/google_firestore_database_project">
    <rdfs:label>project</rdfs:label>
    <rdfs:domain rdf:resource="http://example.org/onto/class/google_firestore_database"/>
    <rdfs:range rdf:resource="http://www.w3.org/2001/XMLSchema#string"/>
  </owl:DatatypeProperty>
  <owl:DatatypeProperty rdf:about="http://example.org/onto/prop/google_firestore_database_tags">
    <rdfs:label>tags</rdfs:label>
    <rdfs:comment>Input only. A map of resource manager tags. Resource manager tag keys
and values have the same definition as resource manager tags.
Keys must be in the format tagKeys/{tag_key_id}, and values are in the format tagValues/456.
The field is ignored when empty. The field is immutable and causes
resource replacement when mutated. To apply tags to an existing resource, see
the 'google_tags_tag_value' resource.</rdfs:comment>
    <rdfs:domain rdf:resource="http://example.org/onto/class/google_firestore_database"/>
    <rdfs:range rdf:resource="http://www.w3.org/2001/XMLSchema#string"/>
  </owl:DatatypeProperty>
  <owl:DatatypeProperty rdf:about="http://example.org/onto/prop/google_firestore_database_type">
    <rdfs:label>type</rdfs:label>
    <rdfs:comment>The type of the database.
See https://cloud.google.com/datastore/docs/firestore-or-datastore
for information about how to choose. Possible values: ["FIRESTORE_NATIVE", "DATASTORE_MODE"]</rdfs:comment>
    <rdfs:domain rdf:resource="http://example.org/onto/class/google_firestore_database"/>
    <rdfs:range rdf:resource="http://www.w3.org/2001/XMLSchema#string"/>
  </owl:DatatypeProperty>
  <owl:DatatypeProperty rdf:about="http://example.org/onto/prop/google_firestore_database_uid">
    <rdfs:label>uid</rdfs:label>
    <rdfs:comment>Output only. The system-generated UUID4 for this Database.</rdfs:comment>
    <rdfs:domain rdf:resource="http://example.org/onto/class/google_firestore_database"/>
    <rdfs:range rdf:resource="http://www.w3.org/2001/XMLSchema#string"/>
  </owl:DatatypeProperty>
  <owl:DatatypeProperty rdf:about="http://example.org/onto/prop/google_firestore_database_update_time">
    <rdfs:label>update_time</rdfs:label>
    <rdfs:comment>Output only. The timestamp at which this database was most recently updated.</rdfs:comment>
    <rdfs:domain rdf:resource="http://example.org/onto/class/google_firestore_database"/>
    <rdfs:range rdf:resource="http://www.w3.org/2001/XMLSchema#string"/>
  </owl:DatatypeProperty>
  <owl:DatatypeProperty rdf:about="http://example.org/onto/prop/google_firestore_database_version_retention_period">
    <rdfs:label>version_retention_period</rdfs:label>
    <rdfs:comment>Output only. The period during which past versions of data are retained in the database.
Any read or query can specify a readTime within this window, and will read the state of the database at that time.
If the PITR feature is enabled, the retention period is 7 days. Otherwise, the retention period is 1 hour.
A duration in seconds with up to nine fractional digits, ending with 's'. Example: "3.5s".</rdfs:comment>
    <rdfs:domain rdf:resource="http://example.org/onto/class/google_firestore_database"/>
    <rdfs:range rdf:resource="http://www.w3.org/2001/XMLSchema#string"/>
  </owl:DatatypeProperty>
  <owl:DatatypeProperty rdf:about="http://example.org/onto/prop/google_firestore_database_active_key_version">
    <rdfs:label>active_key_version</rdfs:label>
    <rdfs:comment>Currently in-use KMS key versions (https://cloud.google.com/kms/docs/resource-hierarchy#key_versions).
During key rotation (https://cloud.google.com/kms/docs/key-rotation), there can be
multiple in-use key versions.

The expected format is
'projects/{project_id}/locations/{kms_location}/keyRings/{key_ring}/cryptoKeys/{crypto_key}/cryptoKeyVersions/{key_version}'.</rdfs:comment>
    <rdfs:domain rdf:resource="http://example.org/onto/class/google_firestore_database"/>
    <rdfs:range rdf:resource="http://www.w3.org/2001/XMLSchema#string"/>
  </owl:DatatypeProperty>
  <owl:DatatypeProperty rdf:about="http://example.org/onto/prop/google_firestore_database_kms_key_name">
    <rdfs:label>kms_key_name</rdfs:label>
    <rdfs:comment>The resource ID of a Cloud KMS key. If set, the database created will
be a Customer-managed Encryption Key (CMEK) database encrypted with
this key. This feature is allowlist only in initial launch.

Only keys in the same location as this database are allowed to be used
for encryption. For Firestore's nam5 multi-region, this corresponds to Cloud KMS
multi-region us. For Firestore's eur3 multi-region, this corresponds to
Cloud KMS multi-region europe. See https://cloud.google.com/kms/docs/locations.

This value should be the KMS key resource ID in the format of
'projects/{project_id}/locations/{kms_location}/keyRings/{key_ring}/cryptoKeys/{crypto_key}'.
How to retrieve this resource ID is listed at
https://cloud.google.com/kms/docs/getting-resource-ids#getting_the_id_for_a_key_and_version.</rdfs:comment>
    <rdfs:domain rdf:resource="http://example.org/onto/class/google_firestore_database"/>
    <rdfs:range rdf:resource="http://www.w3.org/2001/XMLSchema#string"/>
  </owl:DatatypeProperty>
  <owl:DatatypeProperty rdf:about="http://example.org/onto/prop/google_firestore_database_create">
    <rdfs:label>create</rdfs:label>
    <rdfs:domain rdf:resource="http://example.org/onto/class/google_firestore_database"/>
    <rdfs:range rdf:resource="http://www.w3.org/2001/XMLSchema#string"/>
  </owl:DatatypeProperty>
  <owl:DatatypeProperty rdf:about="http://example.org/onto/prop/google_firestore_database_delete">
    <rdfs:label>delete</rdfs:label>
    <rdfs:domain rdf:resource="http://example.org/onto/class/google_firestore_database"/>
    <rdfs:range rdf:resource="http://www.w3.org/2001/XMLSchema#string"/>
  </owl:DatatypeProperty>
  <owl:DatatypeProperty rdf:about="http://example.org/onto/prop/google_firestore_database_update">
    <rdfs:label>update</rdfs:label>
    <rdfs:domain rdf:resource="http://example.org/onto/class/google_firestore_database"/>
    <rdfs:range rdf:resource="http://www.w3.org/2001/XMLSchema#string"/>
  </owl:DatatypeProperty>
</rdf:RDF>
