<?xml version="1.0" encoding="UTF-8"?>
<rdf:RDF
  xmlns:rdf="http://www.w3.org/1999/02/22-rdf-syntax-ns#"
  xmlns:rdfs="http://www.w3.org/2000/01/rdf-schema#"
  xmlns:owl="http://www.w3.org/2002/07/owl#"
  xmlns:xsd="http://www.w3.org/2001/XMLSchema#"
  xml:base="http://example.org/onto/">
  <owl:Class rdf:about="http://example.org/onto/class/google_container_cluster">
    <rdfs:label>google_container_cluster</rdfs:label>
    <rdfs:comment>#
#     ***     AUTO GENERATED CODE    ***    Type: Handwritten     ***
#
# ----------------------------------------------------------------------------
#
#     This code is generated by Magic Modules using the following:
#
#     Source file: https://github.com/GoogleCloudPlatform/magic-modules/tree/main/mmv1/third_party/terraform/website/docs/r/container_cluster.html.markdown
#
#     DO NOT EDIT this file directly. Any changes made to this file will be
#     overwritten during the next generation cycle.
#
# ----------------------------------------------------------------------------
subcategory: "Kubernetes (Container) Engine"
description: |-
  Creates a Google Kubernetes Engine (GKE) cluster.
---</rdfs:comment>
  </owl:Class>
  <owl:DatatypeProperty rdf:about="http://example.org/onto/prop/google_container_cluster_allow_net_admin">
    <rdfs:label>allow_net_admin</rdfs:label>
    <rdfs:comment>Enable NET_ADMIN for this cluster.</rdfs:comment>
    <rdfs:domain rdf:resource="http://example.org/onto/class/google_container_cluster"/>
    <rdfs:range rdf:resource="http://www.w3.org/2001/XMLSchema#string"/>
  </owl:DatatypeProperty>
  <owl:DatatypeProperty rdf:about="http://example.org/onto/prop/google_container_cluster_cluster_ipv4_cidr">
    <rdfs:label>cluster_ipv4_cidr</rdfs:label>
    <rdfs:comment>The IP address range of the Kubernetes pods in this cluster in CIDR notation (e.g. 10.96.0.0/14). Leave blank to have one automatically chosen or specify a /14 block in 10.0.0.0/8. This field will only work for routes-based clusters, where ip_allocation_policy is not defined.</rdfs:comment>
    <rdfs:domain rdf:resource="http://example.org/onto/class/google_container_cluster"/>
    <rdfs:range rdf:resource="http://www.w3.org/2001/XMLSchema#string"/>
  </owl:DatatypeProperty>
  <owl:DatatypeProperty rdf:about="http://example.org/onto/prop/google_container_cluster_datapath_provider">
    <rdfs:label>datapath_provider</rdfs:label>
    <rdfs:comment>The desired datapath provider for this cluster. By default, uses the IPTables-based kube-proxy implementation.</rdfs:comment>
    <rdfs:domain rdf:resource="http://example.org/onto/class/google_container_cluster"/>
    <rdfs:range rdf:resource="http://www.w3.org/2001/XMLSchema#string"/>
  </owl:DatatypeProperty>
  <owl:DatatypeProperty rdf:about="http://example.org/onto/prop/google_container_cluster_default_max_pods_per_node">
    <rdfs:label>default_max_pods_per_node</rdfs:label>
    <rdfs:comment>The default maximum number of pods per node in this cluster. This doesn't work on "routes-based" clusters, clusters that don't have IP Aliasing enabled.</rdfs:comment>
    <rdfs:domain rdf:resource="http://example.org/onto/class/google_container_cluster"/>
    <rdfs:range rdf:resource="http://www.w3.org/2001/XMLSchema#string"/>
  </owl:DatatypeProperty>
  <owl:DatatypeProperty rdf:about="http://example.org/onto/prop/google_container_cluster_deletion_protection">
    <rdfs:label>deletion_protection</rdfs:label>
    <rdfs:comment>When the field is set to true or unset in Terraform state, a terraform apply or terraform destroy that would delete the cluster will fail. When the field is set to false, deleting the cluster is allowed.</rdfs:comment>
    <rdfs:domain rdf:resource="http://example.org/onto/class/google_container_cluster"/>
    <rdfs:range rdf:resource="http://www.w3.org/2001/XMLSchema#string"/>
  </owl:DatatypeProperty>
  <owl:DatatypeProperty rdf:about="http://example.org/onto/prop/google_container_cluster_description">
    <rdfs:label>description</rdfs:label>
    <rdfs:comment>Description of the cluster.</rdfs:comment>
    <rdfs:domain rdf:resource="http://example.org/onto/class/google_container_cluster"/>
    <rdfs:range rdf:resource="http://www.w3.org/2001/XMLSchema#string"/>
  </owl:DatatypeProperty>
  <owl:DatatypeProperty rdf:about="http://example.org/onto/prop/google_container_cluster_disable_l4_lb_firewall_reconciliation">
    <rdfs:label>disable_l4_lb_firewall_reconciliation</rdfs:label>
    <rdfs:comment>Disable L4 load balancer VPC firewalls to enable firewall policies.</rdfs:comment>
    <rdfs:domain rdf:resource="http://example.org/onto/class/google_container_cluster"/>
    <rdfs:range rdf:resource="http://www.w3.org/2001/XMLSchema#string"/>
  </owl:DatatypeProperty>
  <owl:DatatypeProperty rdf:about="http://example.org/onto/prop/google_container_cluster_effective_labels">
    <rdfs:label>effective_labels</rdfs:label>
    <rdfs:comment>All of labels (key/value pairs) present on the resource in GCP, including the labels configured through Terraform, other clients and services.</rdfs:comment>
    <rdfs:domain rdf:resource="http://example.org/onto/class/google_container_cluster"/>
    <rdfs:range rdf:resource="http://www.w3.org/2001/XMLSchema#string"/>
  </owl:DatatypeProperty>
  <owl:DatatypeProperty rdf:about="http://example.org/onto/prop/google_container_cluster_enable_autopilot">
    <rdfs:label>enable_autopilot</rdfs:label>
    <rdfs:comment>Enable Autopilot for this cluster.</rdfs:comment>
    <rdfs:domain rdf:resource="http://example.org/onto/class/google_container_cluster"/>
    <rdfs:range rdf:resource="http://www.w3.org/2001/XMLSchema#string"/>
  </owl:DatatypeProperty>
  <owl:DatatypeProperty rdf:about="http://example.org/onto/prop/google_container_cluster_enable_cilium_clusterwide_network_policy">
    <rdfs:label>enable_cilium_clusterwide_network_policy</rdfs:label>
    <rdfs:comment>Whether Cilium cluster-wide network policy is enabled on this cluster.</rdfs:comment>
    <rdfs:domain rdf:resource="http://example.org/onto/class/google_container_cluster"/>
    <rdfs:range rdf:resource="http://www.w3.org/2001/XMLSchema#string"/>
  </owl:DatatypeProperty>
  <owl:DatatypeProperty rdf:about="http://example.org/onto/prop/google_container_cluster_enable_fqdn_network_policy">
    <rdfs:label>enable_fqdn_network_policy</rdfs:label>
    <rdfs:comment>Whether FQDN Network Policy is enabled on this cluster.</rdfs:comment>
    <rdfs:domain rdf:resource="http://example.org/onto/class/google_container_cluster"/>
    <rdfs:range rdf:resource="http://www.w3.org/2001/XMLSchema#string"/>
  </owl:DatatypeProperty>
  <owl:DatatypeProperty rdf:about="http://example.org/onto/prop/google_container_cluster_enable_intranode_visibility">
    <rdfs:label>enable_intranode_visibility</rdfs:label>
    <rdfs:comment>Whether Intra-node visibility is enabled for this cluster. This makes same node pod to pod traffic visible for VPC network.</rdfs:comment>
    <rdfs:domain rdf:resource="http://example.org/onto/class/google_container_cluster"/>
    <rdfs:range rdf:resource="http://www.w3.org/2001/XMLSchema#string"/>
  </owl:DatatypeProperty>
  <owl:DatatypeProperty rdf:about="http://example.org/onto/prop/google_container_cluster_enable_kubernetes_alpha">
    <rdfs:label>enable_kubernetes_alpha</rdfs:label>
    <rdfs:comment>Whether to enable Kubernetes Alpha features for this cluster. Note that when this option is enabled, the cluster cannot be upgraded and will be automatically deleted after 30 days.</rdfs:comment>
    <rdfs:domain rdf:resource="http://example.org/onto/class/google_container_cluster"/>
    <rdfs:range rdf:resource="http://www.w3.org/2001/XMLSchema#string"/>
  </owl:DatatypeProperty>
  <owl:DatatypeProperty rdf:about="http://example.org/onto/prop/google_container_cluster_enable_l4_ilb_subsetting">
    <rdfs:label>enable_l4_ilb_subsetting</rdfs:label>
    <rdfs:comment>Whether L4ILB Subsetting is enabled for this cluster.</rdfs:comment>
    <rdfs:domain rdf:resource="http://example.org/onto/class/google_container_cluster"/>
    <rdfs:range rdf:resource="http://www.w3.org/2001/XMLSchema#string"/>
  </owl:DatatypeProperty>
  <owl:DatatypeProperty rdf:about="http://example.org/onto/prop/google_container_cluster_enable_legacy_abac">
    <rdfs:label>enable_legacy_abac</rdfs:label>
    <rdfs:comment>Whether the ABAC authorizer is enabled for this cluster. When enabled, identities in the system, including service accounts, nodes, and controllers, will have statically granted permissions beyond those provided by the RBAC configuration or IAM. Defaults to false.</rdfs:comment>
    <rdfs:domain rdf:resource="http://example.org/onto/class/google_container_cluster"/>
    <rdfs:range rdf:resource="http://www.w3.org/2001/XMLSchema#string"/>
  </owl:DatatypeProperty>
  <owl:DatatypeProperty rdf:about="http://example.org/onto/prop/google_container_cluster_enable_multi_networking">
    <rdfs:label>enable_multi_networking</rdfs:label>
    <rdfs:comment>Whether multi-networking is enabled for this cluster.</rdfs:comment>
    <rdfs:domain rdf:resource="http://example.org/onto/class/google_container_cluster"/>
    <rdfs:range rdf:resource="http://www.w3.org/2001/XMLSchema#string"/>
  </owl:DatatypeProperty>
  <owl:DatatypeProperty rdf:about="http://example.org/onto/prop/google_container_cluster_enable_shielded_nodes">
    <rdfs:label>enable_shielded_nodes</rdfs:label>
    <rdfs:comment>Enable Shielded Nodes features on all nodes in this cluster. Defaults to true.</rdfs:comment>
    <rdfs:domain rdf:resource="http://example.org/onto/class/google_container_cluster"/>
    <rdfs:range rdf:resource="http://www.w3.org/2001/XMLSchema#string"/>
  </owl:DatatypeProperty>
  <owl:DatatypeProperty rdf:about="http://example.org/onto/prop/google_container_cluster_enable_tpu">
    <rdfs:label>enable_tpu</rdfs:label>
    <rdfs:comment>Whether to enable Cloud TPU resources in this cluster.</rdfs:comment>
    <rdfs:domain rdf:resource="http://example.org/onto/class/google_container_cluster"/>
    <rdfs:range rdf:resource="http://www.w3.org/2001/XMLSchema#string"/>
  </owl:DatatypeProperty>
  <owl:DatatypeProperty rdf:about="http://example.org/onto/prop/google_container_cluster_endpoint">
    <rdfs:label>endpoint</rdfs:label>
    <rdfs:comment>The IP address of this cluster's Kubernetes master.</rdfs:comment>
    <rdfs:domain rdf:resource="http://example.org/onto/class/google_container_cluster"/>
    <rdfs:range rdf:resource="http://www.w3.org/2001/XMLSchema#string"/>
  </owl:DatatypeProperty>
  <owl:DatatypeProperty rdf:about="http://example.org/onto/prop/google_container_cluster_id">
    <rdfs:label>id</rdfs:label>
    <rdfs:domain rdf:resource="http://example.org/onto/class/google_container_cluster"/>
    <rdfs:range rdf:resource="http://www.w3.org/2001/XMLSchema#string"/>
  </owl:DatatypeProperty>
  <owl:DatatypeProperty rdf:about="http://example.org/onto/prop/google_container_cluster_in_transit_encryption_config">
    <rdfs:label>in_transit_encryption_config</rdfs:label>
    <rdfs:comment>Defines the config of in-transit encryption</rdfs:comment>
    <rdfs:domain rdf:resource="http://example.org/onto/class/google_container_cluster"/>
    <rdfs:range rdf:resource="http://www.w3.org/2001/XMLSchema#string"/>
  </owl:DatatypeProperty>
  <owl:DatatypeProperty rdf:about="http://example.org/onto/prop/google_container_cluster_initial_node_count">
    <rdfs:label>initial_node_count</rdfs:label>
    <rdfs:comment>The number of nodes to create in this cluster's default node pool. In regional or multi-zonal clusters, this is the number of nodes per zone. Must be set if node_pool is not set. If you're using google_container_node_pool objects with no default node pool, you'll need to set this to a value of at least 1, alongside setting remove_default_node_pool to true.</rdfs:comment>
    <rdfs:domain rdf:resource="http://example.org/onto/class/google_container_cluster"/>
    <rdfs:range rdf:resource="http://www.w3.org/2001/XMLSchema#string"/>
  </owl:DatatypeProperty>
  <owl:DatatypeProperty rdf:about="http://example.org/onto/prop/google_container_cluster_label_fingerprint">
    <rdfs:label>label_fingerprint</rdfs:label>
    <rdfs:comment>The fingerprint of the set of labels for this cluster.</rdfs:comment>
    <rdfs:domain rdf:resource="http://example.org/onto/class/google_container_cluster"/>
    <rdfs:range rdf:resource="http://www.w3.org/2001/XMLSchema#string"/>
  </owl:DatatypeProperty>
  <owl:DatatypeProperty rdf:about="http://example.org/onto/prop/google_container_cluster_location">
    <rdfs:label>location</rdfs:label>
    <rdfs:comment>The location (region or zone) in which the cluster master will be created, as well as the default node location. If you specify a zone (such as us-central1-a), the cluster will be a zonal cluster with a single cluster master. If you specify a region (such as us-west1), the cluster will be a regional cluster with multiple masters spread across zones in the region, and with default node locations in those zones as well.</rdfs:comment>
    <rdfs:domain rdf:resource="http://example.org/onto/class/google_container_cluster"/>
    <rdfs:range rdf:resource="http://www.w3.org/2001/XMLSchema#string"/>
  </owl:DatatypeProperty>
  <owl:DatatypeProperty rdf:about="http://example.org/onto/prop/google_container_cluster_logging_service">
    <rdfs:label>logging_service</rdfs:label>
    <rdfs:comment>The logging service that the cluster should write logs to. Available options include logging.googleapis.com(Legacy Stackdriver), logging.googleapis.com/kubernetes(Stackdriver Kubernetes Engine Logging), and none. Defaults to logging.googleapis.com/kubernetes.</rdfs:comment>
    <rdfs:domain rdf:resource="http://example.org/onto/class/google_container_cluster"/>
    <rdfs:range rdf:resource="http://www.w3.org/2001/XMLSchema#string"/>
  </owl:DatatypeProperty>
  <owl:DatatypeProperty rdf:about="http://example.org/onto/prop/google_container_cluster_master_version">
    <rdfs:label>master_version</rdfs:label>
    <rdfs:comment>The current version of the master in the cluster. This may be different than the min_master_version set in the config if the master has been updated by GKE.</rdfs:comment>
    <rdfs:domain rdf:resource="http://example.org/onto/class/google_container_cluster"/>
    <rdfs:range rdf:resource="http://www.w3.org/2001/XMLSchema#string"/>
  </owl:DatatypeProperty>
  <owl:DatatypeProperty rdf:about="http://example.org/onto/prop/google_container_cluster_min_master_version">
    <rdfs:label>min_master_version</rdfs:label>
    <rdfs:comment>The minimum version of the master. GKE will auto-update the master to new versions, so this does not guarantee the current master version--use the read-only master_version field to obtain that. If unset, the cluster's version will be set by GKE to the version of the most recent official release (which is not necessarily the latest version).</rdfs:comment>
    <rdfs:domain rdf:resource="http://example.org/onto/class/google_container_cluster"/>
    <rdfs:range rdf:resource="http://www.w3.org/2001/XMLSchema#string"/>
  </owl:DatatypeProperty>
  <owl:DatatypeProperty rdf:about="http://example.org/onto/prop/google_container_cluster_monitoring_service">
    <rdfs:label>monitoring_service</rdfs:label>
    <rdfs:comment>The monitoring service that the cluster should write metrics to. Automatically send metrics from pods in the cluster to the Google Cloud Monitoring API. VM metrics will be collected by Google Compute Engine regardless of this setting Available options include monitoring.googleapis.com(Legacy Stackdriver), monitoring.googleapis.com/kubernetes(Stackdriver Kubernetes Engine Monitoring), and none. Defaults to monitoring.googleapis.com/kubernetes.</rdfs:comment>
    <rdfs:domain rdf:resource="http://example.org/onto/class/google_container_cluster"/>
    <rdfs:range rdf:resource="http://www.w3.org/2001/XMLSchema#string"/>
  </owl:DatatypeProperty>
  <owl:DatatypeProperty rdf:about="http://example.org/onto/prop/google_container_cluster_name">
    <rdfs:label>name</rdfs:label>
    <rdfs:comment>The name of the cluster, unique within the project and location.</rdfs:comment>
    <rdfs:domain rdf:resource="http://example.org/onto/class/google_container_cluster"/>
    <rdfs:range rdf:resource="http://www.w3.org/2001/XMLSchema#string"/>
  </owl:DatatypeProperty>
  <owl:DatatypeProperty rdf:about="http://example.org/onto/prop/google_container_cluster_network">
    <rdfs:label>network</rdfs:label>
    <rdfs:comment>The name or self_link of the Google Compute Engine network to which the cluster is connected. For Shared VPC, set this to the self link of the shared network.</rdfs:comment>
    <rdfs:domain rdf:resource="http://example.org/onto/class/google_container_cluster"/>
    <rdfs:range rdf:resource="http://www.w3.org/2001/XMLSchema#string"/>
  </owl:DatatypeProperty>
  <owl:DatatypeProperty rdf:about="http://example.org/onto/prop/google_container_cluster_networking_mode">
    <rdfs:label>networking_mode</rdfs:label>
    <rdfs:comment>Determines whether alias IPs or routes will be used for pod IPs in the cluster. Defaults to VPC_NATIVE for new clusters.</rdfs:comment>
    <rdfs:domain rdf:resource="http://example.org/onto/class/google_container_cluster"/>
    <rdfs:range rdf:resource="http://www.w3.org/2001/XMLSchema#string"/>
  </owl:DatatypeProperty>
  <owl:DatatypeProperty rdf:about="http://example.org/onto/prop/google_container_cluster_node_locations">
    <rdfs:label>node_locations</rdfs:label>
    <rdfs:comment>The list of zones in which the cluster's nodes are located. Nodes must be in the region of their regional cluster or in the same region as their cluster's zone for zonal clusters. If this is specified for a zonal cluster, omit the cluster's zone.</rdfs:comment>
    <rdfs:domain rdf:resource="http://example.org/onto/class/google_container_cluster"/>
    <rdfs:range rdf:resource="http://www.w3.org/2001/XMLSchema#string"/>
  </owl:DatatypeProperty>
  <owl:DatatypeProperty rdf:about="http://example.org/onto/prop/google_container_cluster_node_version">
    <rdfs:label>node_version</rdfs:label>
    <rdfs:comment>The Kubernetes version on the nodes. Must either be unset or set to the same value as min_master_version on create. Defaults to the default version set by GKE which is not necessarily the latest version. This only affects nodes in the default node pool. While a fuzzy version can be specified, it's recommended that you specify explicit versions as Terraform will see spurious diffs when fuzzy versions are used. See the google_container_engine_versions data source's version_prefix field to approximate fuzzy versions in a Terraform-compatible way. To update nodes in other node pools, use the version attribute on the node pool.</rdfs:comment>
    <rdfs:domain rdf:resource="http://example.org/onto/class/google_container_cluster"/>
    <rdfs:range rdf:resource="http://www.w3.org/2001/XMLSchema#string"/>
  </owl:DatatypeProperty>
  <owl:DatatypeProperty rdf:about="http://example.org/onto/prop/google_container_cluster_operation">
    <rdfs:label>operation</rdfs:label>
    <rdfs:domain rdf:resource="http://example.org/onto/class/google_container_cluster"/>
    <rdfs:range rdf:resource="http://www.w3.org/2001/XMLSchema#string"/>
  </owl:DatatypeProperty>
  <owl:DatatypeProperty rdf:about="http://example.org/onto/prop/google_container_cluster_private_ipv6_google_access">
    <rdfs:label>private_ipv6_google_access</rdfs:label>
    <rdfs:comment>The desired state of IPv6 connectivity to Google Services. By default, no private IPv6 access to or from Google Services (all access will be via IPv4).</rdfs:comment>
    <rdfs:domain rdf:resource="http://example.org/onto/class/google_container_cluster"/>
    <rdfs:range rdf:resource="http://www.w3.org/2001/XMLSchema#string"/>
  </owl:DatatypeProperty>
  <owl:DatatypeProperty rdf:about="http://example.org/onto/prop/google_container_cluster_project">
    <rdfs:label>project</rdfs:label>
    <rdfs:comment>The ID of the project in which the resource belongs. If it is not provided, the provider project is used.</rdfs:comment>
    <rdfs:domain rdf:resource="http://example.org/onto/class/google_container_cluster"/>
    <rdfs:range rdf:resource="http://www.w3.org/2001/XMLSchema#string"/>
  </owl:DatatypeProperty>
  <owl:DatatypeProperty rdf:about="http://example.org/onto/prop/google_container_cluster_remove_default_node_pool">
    <rdfs:label>remove_default_node_pool</rdfs:label>
    <rdfs:comment>If true, deletes the default node pool upon cluster creation. If you're using google_container_node_pool resources with no default node pool, this should be set to true, alongside setting initial_node_count to at least 1.</rdfs:comment>
    <rdfs:domain rdf:resource="http://example.org/onto/class/google_container_cluster"/>
    <rdfs:range rdf:resource="http://www.w3.org/2001/XMLSchema#string"/>
  </owl:DatatypeProperty>
  <owl:DatatypeProperty rdf:about="http://example.org/onto/prop/google_container_cluster_resource_labels">
    <rdfs:label>resource_labels</rdfs:label>
    <rdfs:comment>The GCE resource labels (a map of key/value pairs) to be applied to the cluster.

				**Note**: This field is non-authoritative, and will only manage the labels present in your configuration.
				Please refer to the field 'effective_labels' for all of the labels present on the resource.</rdfs:comment>
    <rdfs:domain rdf:resource="http://example.org/onto/class/google_container_cluster"/>
    <rdfs:range rdf:resource="http://www.w3.org/2001/XMLSchema#string"/>
  </owl:DatatypeProperty>
  <owl:DatatypeProperty rdf:about="http://example.org/onto/prop/google_container_cluster_self_link">
    <rdfs:label>self_link</rdfs:label>
    <rdfs:comment>Server-defined URL for the resource.</rdfs:comment>
    <rdfs:domain rdf:resource="http://example.org/onto/class/google_container_cluster"/>
    <rdfs:range rdf:resource="http://www.w3.org/2001/XMLSchema#string"/>
  </owl:DatatypeProperty>
  <owl:DatatypeProperty rdf:about="http://example.org/onto/prop/google_container_cluster_services_ipv4_cidr">
    <rdfs:label>services_ipv4_cidr</rdfs:label>
    <rdfs:comment>The IP address range of the Kubernetes services in this cluster, in CIDR notation (e.g. 1.2.3.4/29). Service addresses are typically put in the last /16 from the container CIDR.</rdfs:comment>
    <rdfs:domain rdf:resource="http://example.org/onto/class/google_container_cluster"/>
    <rdfs:range rdf:resource="http://www.w3.org/2001/XMLSchema#string"/>
  </owl:DatatypeProperty>
  <owl:DatatypeProperty rdf:about="http://example.org/onto/prop/google_container_cluster_subnetwork">
    <rdfs:label>subnetwork</rdfs:label>
    <rdfs:comment>The name or self_link of the Google Compute Engine subnetwork in which the cluster's instances are launched.</rdfs:comment>
    <rdfs:domain rdf:resource="http://example.org/onto/class/google_container_cluster"/>
    <rdfs:range rdf:resource="http://www.w3.org/2001/XMLSchema#string"/>
  </owl:DatatypeProperty>
  <owl:DatatypeProperty rdf:about="http://example.org/onto/prop/google_container_cluster_terraform_labels">
    <rdfs:label>terraform_labels</rdfs:label>
    <rdfs:comment>The combination of labels configured directly on the resource and default labels configured on the provider.</rdfs:comment>
    <rdfs:domain rdf:resource="http://example.org/onto/class/google_container_cluster"/>
    <rdfs:range rdf:resource="http://www.w3.org/2001/XMLSchema#string"/>
  </owl:DatatypeProperty>
  <owl:DatatypeProperty rdf:about="http://example.org/onto/prop/google_container_cluster_tpu_ipv4_cidr_block">
    <rdfs:label>tpu_ipv4_cidr_block</rdfs:label>
    <rdfs:comment>The IP address range of the Cloud TPUs in this cluster, in CIDR notation (e.g. 1.2.3.4/29).</rdfs:comment>
    <rdfs:domain rdf:resource="http://example.org/onto/class/google_container_cluster"/>
    <rdfs:range rdf:resource="http://www.w3.org/2001/XMLSchema#string"/>
  </owl:DatatypeProperty>
  <owl:DatatypeProperty rdf:about="http://example.org/onto/prop/google_container_cluster_disabled">
    <rdfs:label>disabled</rdfs:label>
    <rdfs:domain rdf:resource="http://example.org/onto/class/google_container_cluster"/>
    <rdfs:range rdf:resource="http://www.w3.org/2001/XMLSchema#string"/>
  </owl:DatatypeProperty>
  <owl:DatatypeProperty rdf:about="http://example.org/onto/prop/google_container_cluster_load_balancer_type">
    <rdfs:label>load_balancer_type</rdfs:label>
    <rdfs:domain rdf:resource="http://example.org/onto/class/google_container_cluster"/>
    <rdfs:range rdf:resource="http://www.w3.org/2001/XMLSchema#string"/>
  </owl:DatatypeProperty>
  <owl:DatatypeProperty rdf:about="http://example.org/onto/prop/google_container_cluster_enabled">
    <rdfs:label>enabled</rdfs:label>
    <rdfs:domain rdf:resource="http://example.org/onto/class/google_container_cluster"/>
    <rdfs:range rdf:resource="http://www.w3.org/2001/XMLSchema#string"/>
  </owl:DatatypeProperty>
  <owl:DatatypeProperty rdf:about="http://example.org/onto/prop/google_container_cluster_enabled">
    <rdfs:label>enabled</rdfs:label>
    <rdfs:domain rdf:resource="http://example.org/onto/class/google_container_cluster"/>
    <rdfs:range rdf:resource="http://www.w3.org/2001/XMLSchema#string"/>
  </owl:DatatypeProperty>
  <owl:DatatypeProperty rdf:about="http://example.org/onto/prop/google_container_cluster_enabled">
    <rdfs:label>enabled</rdfs:label>
    <rdfs:domain rdf:resource="http://example.org/onto/class/google_container_cluster"/>
    <rdfs:range rdf:resource="http://www.w3.org/2001/XMLSchema#string"/>
  </owl:DatatypeProperty>
  <owl:DatatypeProperty rdf:about="http://example.org/onto/prop/google_container_cluster_enabled">
    <rdfs:label>enabled</rdfs:label>
    <rdfs:domain rdf:resource="http://example.org/onto/class/google_container_cluster"/>
    <rdfs:range rdf:resource="http://www.w3.org/2001/XMLSchema#string"/>
  </owl:DatatypeProperty>
  <owl:DatatypeProperty rdf:about="http://example.org/onto/prop/google_container_cluster_enabled">
    <rdfs:label>enabled</rdfs:label>
    <rdfs:domain rdf:resource="http://example.org/onto/class/google_container_cluster"/>
    <rdfs:range rdf:resource="http://www.w3.org/2001/XMLSchema#string"/>
  </owl:DatatypeProperty>
  <owl:DatatypeProperty rdf:about="http://example.org/onto/prop/google_container_cluster_enabled">
    <rdfs:label>enabled</rdfs:label>
    <rdfs:domain rdf:resource="http://example.org/onto/class/google_container_cluster"/>
    <rdfs:range rdf:resource="http://www.w3.org/2001/XMLSchema#string"/>
  </owl:DatatypeProperty>
  <owl:DatatypeProperty rdf:about="http://example.org/onto/prop/google_container_cluster_disabled">
    <rdfs:label>disabled</rdfs:label>
    <rdfs:domain rdf:resource="http://example.org/onto/class/google_container_cluster"/>
    <rdfs:range rdf:resource="http://www.w3.org/2001/XMLSchema#string"/>
  </owl:DatatypeProperty>
  <owl:DatatypeProperty rdf:about="http://example.org/onto/prop/google_container_cluster_disabled">
    <rdfs:label>disabled</rdfs:label>
    <rdfs:domain rdf:resource="http://example.org/onto/class/google_container_cluster"/>
    <rdfs:range rdf:resource="http://www.w3.org/2001/XMLSchema#string"/>
  </owl:DatatypeProperty>
  <owl:DatatypeProperty rdf:about="http://example.org/onto/prop/google_container_cluster_enable_legacy_lustre_port">
    <rdfs:label>enable_legacy_lustre_port</rdfs:label>
    <rdfs:comment>If set to true, the Lustre CSI driver will initialize LNet (the virtual network layer for Lustre kernel module) using port 6988.
										This flag is required to workaround a port conflict with the gke-metadata-server on GKE nodes.</rdfs:comment>
    <rdfs:domain rdf:resource="http://example.org/onto/class/google_container_cluster"/>
    <rdfs:range rdf:resource="http://www.w3.org/2001/XMLSchema#string"/>
  </owl:DatatypeProperty>
  <owl:DatatypeProperty rdf:about="http://example.org/onto/prop/google_container_cluster_enabled">
    <rdfs:label>enabled</rdfs:label>
    <rdfs:comment>Whether the Lustre CSI driver is enabled for this cluster.</rdfs:comment>
    <rdfs:domain rdf:resource="http://example.org/onto/class/google_container_cluster"/>
    <rdfs:range rdf:resource="http://www.w3.org/2001/XMLSchema#string"/>
  </owl:DatatypeProperty>
  <owl:DatatypeProperty rdf:about="http://example.org/onto/prop/google_container_cluster_disabled">
    <rdfs:label>disabled</rdfs:label>
    <rdfs:domain rdf:resource="http://example.org/onto/class/google_container_cluster"/>
    <rdfs:range rdf:resource="http://www.w3.org/2001/XMLSchema#string"/>
  </owl:DatatypeProperty>
  <owl:DatatypeProperty rdf:about="http://example.org/onto/prop/google_container_cluster_enabled">
    <rdfs:label>enabled</rdfs:label>
    <rdfs:domain rdf:resource="http://example.org/onto/class/google_container_cluster"/>
    <rdfs:range rdf:resource="http://www.w3.org/2001/XMLSchema#string"/>
  </owl:DatatypeProperty>
  <owl:DatatypeProperty rdf:about="http://example.org/onto/prop/google_container_cluster_enabled">
    <rdfs:label>enabled</rdfs:label>
    <rdfs:domain rdf:resource="http://example.org/onto/class/google_container_cluster"/>
    <rdfs:range rdf:resource="http://www.w3.org/2001/XMLSchema#string"/>
  </owl:DatatypeProperty>
  <owl:DatatypeProperty rdf:about="http://example.org/onto/prop/google_container_cluster_enabled">
    <rdfs:label>enabled</rdfs:label>
    <rdfs:domain rdf:resource="http://example.org/onto/class/google_container_cluster"/>
    <rdfs:range rdf:resource="http://www.w3.org/2001/XMLSchema#string"/>
  </owl:DatatypeProperty>
  <owl:DatatypeProperty rdf:about="http://example.org/onto/prop/google_container_cluster_enabled">
    <rdfs:label>enabled</rdfs:label>
    <rdfs:domain rdf:resource="http://example.org/onto/class/google_container_cluster"/>
    <rdfs:range rdf:resource="http://www.w3.org/2001/XMLSchema#string"/>
  </owl:DatatypeProperty>
  <owl:DatatypeProperty rdf:about="http://example.org/onto/prop/google_container_cluster_enabled">
    <rdfs:label>enabled</rdfs:label>
    <rdfs:domain rdf:resource="http://example.org/onto/class/google_container_cluster"/>
    <rdfs:range rdf:resource="http://www.w3.org/2001/XMLSchema#string"/>
  </owl:DatatypeProperty>
  <owl:DatatypeProperty rdf:about="http://example.org/onto/prop/google_container_cluster_mode">
    <rdfs:label>mode</rdfs:label>
    <rdfs:comment>Setting this to LIMITED will restrict authentication of anonymous users to health check endpoints only.
 Accepted values are:
* ENABLED: Authentication of anonymous users is enabled for all endpoints.
* LIMITED: Anonymous access is only allowed for health check endpoints.</rdfs:comment>
    <rdfs:domain rdf:resource="http://example.org/onto/class/google_container_cluster"/>
    <rdfs:range rdf:resource="http://www.w3.org/2001/XMLSchema#string"/>
  </owl:DatatypeProperty>
  <owl:DatatypeProperty rdf:about="http://example.org/onto/prop/google_container_cluster_security_group">
    <rdfs:label>security_group</rdfs:label>
    <rdfs:comment>The name of the RBAC security group for use with Google security groups in Kubernetes RBAC. Group name must be in format gke-security-groups@yourdomain.com.</rdfs:comment>
    <rdfs:domain rdf:resource="http://example.org/onto/class/google_container_cluster"/>
    <rdfs:range rdf:resource="http://www.w3.org/2001/XMLSchema#string"/>
  </owl:DatatypeProperty>
  <owl:DatatypeProperty rdf:about="http://example.org/onto/prop/google_container_cluster_enabled">
    <rdfs:label>enabled</rdfs:label>
    <rdfs:comment>Enable Binary Authorization for this cluster.</rdfs:comment>
    <rdfs:domain rdf:resource="http://example.org/onto/class/google_container_cluster"/>
    <rdfs:range rdf:resource="http://www.w3.org/2001/XMLSchema#string"/>
  </owl:DatatypeProperty>
  <owl:DatatypeProperty rdf:about="http://example.org/onto/prop/google_container_cluster_evaluation_mode">
    <rdfs:label>evaluation_mode</rdfs:label>
    <rdfs:comment>Mode of operation for Binary Authorization policy evaluation.</rdfs:comment>
    <rdfs:domain rdf:resource="http://example.org/onto/class/google_container_cluster"/>
    <rdfs:range rdf:resource="http://www.w3.org/2001/XMLSchema#string"/>
  </owl:DatatypeProperty>
  <owl:DatatypeProperty rdf:about="http://example.org/onto/prop/google_container_cluster_auto_provisioning_locations">
    <rdfs:label>auto_provisioning_locations</rdfs:label>
    <rdfs:comment>The list of Google Compute Engine zones in which the NodePool's nodes can be created by NAP.</rdfs:comment>
    <rdfs:domain rdf:resource="http://example.org/onto/class/google_container_cluster"/>
    <rdfs:range rdf:resource="http://www.w3.org/2001/XMLSchema#string"/>
  </owl:DatatypeProperty>
  <owl:DatatypeProperty rdf:about="http://example.org/onto/prop/google_container_cluster_autoscaling_profile">
    <rdfs:label>autoscaling_profile</rdfs:label>
    <rdfs:comment>Configuration options for the Autoscaling profile feature, which lets you choose whether the cluster autoscaler should optimize for resource utilization or resource availability when deciding to remove nodes from a cluster. Can be BALANCED or OPTIMIZE_UTILIZATION. Defaults to BALANCED.</rdfs:comment>
    <rdfs:domain rdf:resource="http://example.org/onto/class/google_container_cluster"/>
    <rdfs:range rdf:resource="http://www.w3.org/2001/XMLSchema#string"/>
  </owl:DatatypeProperty>
  <owl:DatatypeProperty rdf:about="http://example.org/onto/prop/google_container_cluster_default_compute_class_enabled">
    <rdfs:label>default_compute_class_enabled</rdfs:label>
    <rdfs:comment>Specifies whether default compute class behaviour is enabled. If enabled, cluster autoscaler will use Compute Class with name default for all the workloads, if not overriden.</rdfs:comment>
    <rdfs:domain rdf:resource="http://example.org/onto/class/google_container_cluster"/>
    <rdfs:range rdf:resource="http://www.w3.org/2001/XMLSchema#string"/>
  </owl:DatatypeProperty>
  <owl:DatatypeProperty rdf:about="http://example.org/onto/prop/google_container_cluster_enabled">
    <rdfs:label>enabled</rdfs:label>
    <rdfs:comment>Whether node auto-provisioning is enabled. Resource limits for cpu and memory must be defined to enable node auto-provisioning.</rdfs:comment>
    <rdfs:domain rdf:resource="http://example.org/onto/class/google_container_cluster"/>
    <rdfs:range rdf:resource="http://www.w3.org/2001/XMLSchema#string"/>
  </owl:DatatypeProperty>
  <owl:DatatypeProperty rdf:about="http://example.org/onto/prop/google_container_cluster_boot_disk_kms_key">
    <rdfs:label>boot_disk_kms_key</rdfs:label>
    <rdfs:comment>The Customer Managed Encryption Key used to encrypt the boot disk attached to each node in the node pool.</rdfs:comment>
    <rdfs:domain rdf:resource="http://example.org/onto/class/google_container_cluster"/>
    <rdfs:range rdf:resource="http://www.w3.org/2001/XMLSchema#string"/>
  </owl:DatatypeProperty>
  <owl:DatatypeProperty rdf:about="http://example.org/onto/prop/google_container_cluster_disk_size">
    <rdfs:label>disk_size</rdfs:label>
    <rdfs:comment>Size of the disk attached to each node, specified in GB. The smallest allowed disk size is 10GB.</rdfs:comment>
    <rdfs:domain rdf:resource="http://example.org/onto/class/google_container_cluster"/>
    <rdfs:range rdf:resource="http://www.w3.org/2001/XMLSchema#string"/>
  </owl:DatatypeProperty>
  <owl:DatatypeProperty rdf:about="http://example.org/onto/prop/google_container_cluster_disk_type">
    <rdfs:label>disk_type</rdfs:label>
    <rdfs:comment>Type of the disk attached to each node.</rdfs:comment>
    <rdfs:domain rdf:resource="http://example.org/onto/class/google_container_cluster"/>
    <rdfs:range rdf:resource="http://www.w3.org/2001/XMLSchema#string"/>
  </owl:DatatypeProperty>
  <owl:DatatypeProperty rdf:about="http://example.org/onto/prop/google_container_cluster_image_type">
    <rdfs:label>image_type</rdfs:label>
    <rdfs:comment>The default image type used by NAP once a new node pool is being created.</rdfs:comment>
    <rdfs:domain rdf:resource="http://example.org/onto/class/google_container_cluster"/>
    <rdfs:range rdf:resource="http://www.w3.org/2001/XMLSchema#string"/>
  </owl:DatatypeProperty>
  <owl:DatatypeProperty rdf:about="http://example.org/onto/prop/google_container_cluster_min_cpu_platform">
    <rdfs:label>min_cpu_platform</rdfs:label>
    <rdfs:comment>Minimum CPU platform to be used by this instance. The instance may be scheduled on the specified or newer CPU platform. Applicable values are the friendly names of CPU platforms, such as Intel Haswell.</rdfs:comment>
    <rdfs:domain rdf:resource="http://example.org/onto/class/google_container_cluster"/>
    <rdfs:range rdf:resource="http://www.w3.org/2001/XMLSchema#string"/>
  </owl:DatatypeProperty>
  <owl:DatatypeProperty rdf:about="http://example.org/onto/prop/google_container_cluster_oauth_scopes">
    <rdfs:label>oauth_scopes</rdfs:label>
    <rdfs:comment>Scopes that are used by NAP when creating node pools.</rdfs:comment>
    <rdfs:domain rdf:resource="http://example.org/onto/class/google_container_cluster"/>
    <rdfs:range rdf:resource="http://www.w3.org/2001/XMLSchema#string"/>
  </owl:DatatypeProperty>
  <owl:DatatypeProperty rdf:about="http://example.org/onto/prop/google_container_cluster_service_account">
    <rdfs:label>service_account</rdfs:label>
    <rdfs:comment>The Google Cloud Platform Service Account to be used by the node VMs.</rdfs:comment>
    <rdfs:domain rdf:resource="http://example.org/onto/class/google_container_cluster"/>
    <rdfs:range rdf:resource="http://www.w3.org/2001/XMLSchema#string"/>
  </owl:DatatypeProperty>
  <owl:DatatypeProperty rdf:about="http://example.org/onto/prop/google_container_cluster_auto_repair">
    <rdfs:label>auto_repair</rdfs:label>
    <rdfs:comment>Specifies whether the node auto-repair is enabled for the node pool. If enabled, the nodes in this node pool will be monitored and, if they fail health checks too many times, an automatic repair action will be triggered.</rdfs:comment>
    <rdfs:domain rdf:resource="http://example.org/onto/class/google_container_cluster"/>
    <rdfs:range rdf:resource="http://www.w3.org/2001/XMLSchema#string"/>
  </owl:DatatypeProperty>
  <owl:DatatypeProperty rdf:about="http://example.org/onto/prop/google_container_cluster_auto_upgrade">
    <rdfs:label>auto_upgrade</rdfs:label>
    <rdfs:comment>Specifies whether node auto-upgrade is enabled for the node pool. If enabled, node auto-upgrade helps keep the nodes in your node pool up to date with the latest release version of Kubernetes.</rdfs:comment>
    <rdfs:domain rdf:resource="http://example.org/onto/class/google_container_cluster"/>
    <rdfs:range rdf:resource="http://www.w3.org/2001/XMLSchema#string"/>
  </owl:DatatypeProperty>
  <owl:DatatypeProperty rdf:about="http://example.org/onto/prop/google_container_cluster_upgrade_options">
    <rdfs:label>upgrade_options</rdfs:label>
    <rdfs:comment>Specifies the Auto Upgrade knobs for the node pool.</rdfs:comment>
    <rdfs:domain rdf:resource="http://example.org/onto/class/google_container_cluster"/>
    <rdfs:range rdf:resource="http://www.w3.org/2001/XMLSchema#string"/>
  </owl:DatatypeProperty>
  <owl:DatatypeProperty rdf:about="http://example.org/onto/prop/google_container_cluster_enable_integrity_monitoring">
    <rdfs:label>enable_integrity_monitoring</rdfs:label>
    <rdfs:comment>Defines whether the instance has integrity monitoring enabled.</rdfs:comment>
    <rdfs:domain rdf:resource="http://example.org/onto/class/google_container_cluster"/>
    <rdfs:range rdf:resource="http://www.w3.org/2001/XMLSchema#string"/>
  </owl:DatatypeProperty>
  <owl:DatatypeProperty rdf:about="http://example.org/onto/prop/google_container_cluster_enable_secure_boot">
    <rdfs:label>enable_secure_boot</rdfs:label>
    <rdfs:comment>Defines whether the instance has Secure Boot enabled.</rdfs:comment>
    <rdfs:domain rdf:resource="http://example.org/onto/class/google_container_cluster"/>
    <rdfs:range rdf:resource="http://www.w3.org/2001/XMLSchema#string"/>
  </owl:DatatypeProperty>
  <owl:DatatypeProperty rdf:about="http://example.org/onto/prop/google_container_cluster_max_surge">
    <rdfs:label>max_surge</rdfs:label>
    <rdfs:comment>The maximum number of nodes that can be created beyond the current size of the node pool during the upgrade process.</rdfs:comment>
    <rdfs:domain rdf:resource="http://example.org/onto/class/google_container_cluster"/>
    <rdfs:range rdf:resource="http://www.w3.org/2001/XMLSchema#string"/>
  </owl:DatatypeProperty>
  <owl:DatatypeProperty rdf:about="http://example.org/onto/prop/google_container_cluster_max_unavailable">
    <rdfs:label>max_unavailable</rdfs:label>
    <rdfs:comment>The maximum number of nodes that can be simultaneously unavailable during the upgrade process.</rdfs:comment>
    <rdfs:domain rdf:resource="http://example.org/onto/class/google_container_cluster"/>
    <rdfs:range rdf:resource="http://www.w3.org/2001/XMLSchema#string"/>
  </owl:DatatypeProperty>
  <owl:DatatypeProperty rdf:about="http://example.org/onto/prop/google_container_cluster_strategy">
    <rdfs:label>strategy</rdfs:label>
    <rdfs:comment>Update strategy of the node pool.</rdfs:comment>
    <rdfs:domain rdf:resource="http://example.org/onto/class/google_container_cluster"/>
    <rdfs:range rdf:resource="http://www.w3.org/2001/XMLSchema#string"/>
  </owl:DatatypeProperty>
  <owl:DatatypeProperty rdf:about="http://example.org/onto/prop/google_container_cluster_node_pool_soak_duration">
    <rdfs:label>node_pool_soak_duration</rdfs:label>
    <rdfs:comment>Time needed after draining entire blue pool. After this period, blue pool will be cleaned up.

																A duration in seconds with up to nine fractional digits, ending with 's'. Example: "3.5s".</rdfs:comment>
    <rdfs:domain rdf:resource="http://example.org/onto/class/google_container_cluster"/>
    <rdfs:range rdf:resource="http://www.w3.org/2001/XMLSchema#string"/>
  </owl:DatatypeProperty>
  <owl:DatatypeProperty rdf:about="http://example.org/onto/prop/google_container_cluster_batch_node_count">
    <rdfs:label>batch_node_count</rdfs:label>
    <rdfs:comment>Number of blue nodes to drain in a batch.</rdfs:comment>
    <rdfs:domain rdf:resource="http://example.org/onto/class/google_container_cluster"/>
    <rdfs:range rdf:resource="http://www.w3.org/2001/XMLSchema#string"/>
  </owl:DatatypeProperty>
  <owl:DatatypeProperty rdf:about="http://example.org/onto/prop/google_container_cluster_batch_percentage">
    <rdfs:label>batch_percentage</rdfs:label>
    <rdfs:comment>Percentage of the bool pool nodes to drain in a batch. The range of this field should be (0.0, 1.0].</rdfs:comment>
    <rdfs:domain rdf:resource="http://example.org/onto/class/google_container_cluster"/>
    <rdfs:range rdf:resource="http://www.w3.org/2001/XMLSchema#string"/>
  </owl:DatatypeProperty>
  <owl:DatatypeProperty rdf:about="http://example.org/onto/prop/google_container_cluster_batch_soak_duration">
    <rdfs:label>batch_soak_duration</rdfs:label>
    <rdfs:comment>Soak time after each batch gets drained.

																			A duration in seconds with up to nine fractional digits, ending with 's'. Example: "3.5s".</rdfs:comment>
    <rdfs:domain rdf:resource="http://example.org/onto/class/google_container_cluster"/>
    <rdfs:range rdf:resource="http://www.w3.org/2001/XMLSchema#string"/>
  </owl:DatatypeProperty>
  <owl:DatatypeProperty rdf:about="http://example.org/onto/prop/google_container_cluster_maximum">
    <rdfs:label>maximum</rdfs:label>
    <rdfs:comment>Maximum amount of the resource in the cluster.</rdfs:comment>
    <rdfs:domain rdf:resource="http://example.org/onto/class/google_container_cluster"/>
    <rdfs:range rdf:resource="http://www.w3.org/2001/XMLSchema#string"/>
  </owl:DatatypeProperty>
  <owl:DatatypeProperty rdf:about="http://example.org/onto/prop/google_container_cluster_minimum">
    <rdfs:label>minimum</rdfs:label>
    <rdfs:comment>Minimum amount of the resource in the cluster.</rdfs:comment>
    <rdfs:domain rdf:resource="http://example.org/onto/class/google_container_cluster"/>
    <rdfs:range rdf:resource="http://www.w3.org/2001/XMLSchema#string"/>
  </owl:DatatypeProperty>
  <owl:DatatypeProperty rdf:about="http://example.org/onto/prop/google_container_cluster_resource_type">
    <rdfs:label>resource_type</rdfs:label>
    <rdfs:comment>The type of the resource. For example, cpu and memory. See the guide to using Node Auto-Provisioning for a list of types.</rdfs:comment>
    <rdfs:domain rdf:resource="http://example.org/onto/class/google_container_cluster"/>
    <rdfs:range rdf:resource="http://www.w3.org/2001/XMLSchema#string"/>
  </owl:DatatypeProperty>
  <owl:DatatypeProperty rdf:about="http://example.org/onto/prop/google_container_cluster_confidential_instance_type">
    <rdfs:label>confidential_instance_type</rdfs:label>
    <rdfs:comment>Defines the type of technology used by the confidential node.</rdfs:comment>
    <rdfs:domain rdf:resource="http://example.org/onto/class/google_container_cluster"/>
    <rdfs:range rdf:resource="http://www.w3.org/2001/XMLSchema#string"/>
  </owl:DatatypeProperty>
  <owl:DatatypeProperty rdf:about="http://example.org/onto/prop/google_container_cluster_enabled">
    <rdfs:label>enabled</rdfs:label>
    <rdfs:comment>Whether Confidential Nodes feature is enabled for all nodes in this cluster.</rdfs:comment>
    <rdfs:domain rdf:resource="http://example.org/onto/class/google_container_cluster"/>
    <rdfs:range rdf:resource="http://www.w3.org/2001/XMLSchema#string"/>
  </owl:DatatypeProperty>
  <owl:DatatypeProperty rdf:about="http://example.org/onto/prop/google_container_cluster_allow_external_traffic">
    <rdfs:label>allow_external_traffic</rdfs:label>
    <rdfs:comment>Controls whether user traffic is allowed over this endpoint. Note that GCP-managed services may still use the endpoint even if this is false.</rdfs:comment>
    <rdfs:domain rdf:resource="http://example.org/onto/class/google_container_cluster"/>
    <rdfs:range rdf:resource="http://www.w3.org/2001/XMLSchema#string"/>
  </owl:DatatypeProperty>
  <owl:DatatypeProperty rdf:about="http://example.org/onto/prop/google_container_cluster_endpoint">
    <rdfs:label>endpoint</rdfs:label>
    <rdfs:comment>The cluster's DNS endpoint.</rdfs:comment>
    <rdfs:domain rdf:resource="http://example.org/onto/class/google_container_cluster"/>
    <rdfs:range rdf:resource="http://www.w3.org/2001/XMLSchema#string"/>
  </owl:DatatypeProperty>
  <owl:DatatypeProperty rdf:about="http://example.org/onto/prop/google_container_cluster_enabled">
    <rdfs:label>enabled</rdfs:label>
    <rdfs:comment>Controls whether to allow direct IP access.</rdfs:comment>
    <rdfs:domain rdf:resource="http://example.org/onto/class/google_container_cluster"/>
    <rdfs:range rdf:resource="http://www.w3.org/2001/XMLSchema#string"/>
  </owl:DatatypeProperty>
  <owl:DatatypeProperty rdf:about="http://example.org/onto/prop/google_container_cluster_enabled">
    <rdfs:label>enabled</rdfs:label>
    <rdfs:comment>Whether to enable GKE cost allocation. When you enable GKE cost allocation, the cluster name and namespace of your GKE workloads appear in the labels field of the billing export to BigQuery. Defaults to false.</rdfs:comment>
    <rdfs:domain rdf:resource="http://example.org/onto/class/google_container_cluster"/>
    <rdfs:range rdf:resource="http://www.w3.org/2001/XMLSchema#string"/>
  </owl:DatatypeProperty>
  <owl:DatatypeProperty rdf:about="http://example.org/onto/prop/google_container_cluster_key_name">
    <rdfs:label>key_name</rdfs:label>
    <rdfs:comment>The key to use to encrypt/decrypt secrets.</rdfs:comment>
    <rdfs:domain rdf:resource="http://example.org/onto/class/google_container_cluster"/>
    <rdfs:range rdf:resource="http://www.w3.org/2001/XMLSchema#string"/>
  </owl:DatatypeProperty>
  <owl:DatatypeProperty rdf:about="http://example.org/onto/prop/google_container_cluster_state">
    <rdfs:label>state</rdfs:label>
    <rdfs:comment>ENCRYPTED or DECRYPTED.</rdfs:comment>
    <rdfs:domain rdf:resource="http://example.org/onto/class/google_container_cluster"/>
    <rdfs:range rdf:resource="http://www.w3.org/2001/XMLSchema#string"/>
  </owl:DatatypeProperty>
  <owl:DatatypeProperty rdf:about="http://example.org/onto/prop/google_container_cluster_disabled">
    <rdfs:label>disabled</rdfs:label>
    <rdfs:comment>When disabled is set to false, default IP masquerade rules will be applied to the nodes to prevent sNAT on cluster internal traffic.</rdfs:comment>
    <rdfs:domain rdf:resource="http://example.org/onto/class/google_container_cluster"/>
    <rdfs:range rdf:resource="http://www.w3.org/2001/XMLSchema#string"/>
  </owl:DatatypeProperty>
  <owl:DatatypeProperty rdf:about="http://example.org/onto/prop/google_container_cluster_additive_vpc_scope_dns_domain">
    <rdfs:label>additive_vpc_scope_dns_domain</rdfs:label>
    <rdfs:comment>Enable additive VPC scope DNS in a GKE cluster.</rdfs:comment>
    <rdfs:domain rdf:resource="http://example.org/onto/class/google_container_cluster"/>
    <rdfs:range rdf:resource="http://www.w3.org/2001/XMLSchema#string"/>
  </owl:DatatypeProperty>
  <owl:DatatypeProperty rdf:about="http://example.org/onto/prop/google_container_cluster_cluster_dns">
    <rdfs:label>cluster_dns</rdfs:label>
    <rdfs:comment>Which in-cluster DNS provider should be used.</rdfs:comment>
    <rdfs:domain rdf:resource="http://example.org/onto/class/google_container_cluster"/>
    <rdfs:range rdf:resource="http://www.w3.org/2001/XMLSchema#string"/>
  </owl:DatatypeProperty>
  <owl:DatatypeProperty rdf:about="http://example.org/onto/prop/google_container_cluster_cluster_dns_domain">
    <rdfs:label>cluster_dns_domain</rdfs:label>
    <rdfs:comment>The suffix used for all cluster service records.</rdfs:comment>
    <rdfs:domain rdf:resource="http://example.org/onto/class/google_container_cluster"/>
    <rdfs:range rdf:resource="http://www.w3.org/2001/XMLSchema#string"/>
  </owl:DatatypeProperty>
  <owl:DatatypeProperty rdf:about="http://example.org/onto/prop/google_container_cluster_cluster_dns_scope">
    <rdfs:label>cluster_dns_scope</rdfs:label>
    <rdfs:comment>The scope of access to cluster DNS records.</rdfs:comment>
    <rdfs:domain rdf:resource="http://example.org/onto/class/google_container_cluster"/>
    <rdfs:range rdf:resource="http://www.w3.org/2001/XMLSchema#string"/>
  </owl:DatatypeProperty>
  <owl:DatatypeProperty rdf:about="http://example.org/onto/prop/google_container_cluster_enabled_apis">
    <rdfs:label>enabled_apis</rdfs:label>
    <rdfs:comment>Enabled Kubernetes Beta APIs.</rdfs:comment>
    <rdfs:domain rdf:resource="http://example.org/onto/class/google_container_cluster"/>
    <rdfs:range rdf:resource="http://www.w3.org/2001/XMLSchema#string"/>
  </owl:DatatypeProperty>
  <owl:DatatypeProperty rdf:about="http://example.org/onto/prop/google_container_cluster_cluster_tier">
    <rdfs:label>cluster_tier</rdfs:label>
    <rdfs:comment>Indicates the effective cluster tier. Available options include STANDARD and ENTERPRISE.</rdfs:comment>
    <rdfs:domain rdf:resource="http://example.org/onto/class/google_container_cluster"/>
    <rdfs:range rdf:resource="http://www.w3.org/2001/XMLSchema#string"/>
  </owl:DatatypeProperty>
  <owl:DatatypeProperty rdf:about="http://example.org/onto/prop/google_container_cluster_desired_tier">
    <rdfs:label>desired_tier</rdfs:label>
    <rdfs:comment>Indicates the desired cluster tier. Available options include STANDARD and ENTERPRISE.</rdfs:comment>
    <rdfs:domain rdf:resource="http://example.org/onto/class/google_container_cluster"/>
    <rdfs:range rdf:resource="http://www.w3.org/2001/XMLSchema#string"/>
  </owl:DatatypeProperty>
  <owl:DatatypeProperty rdf:about="http://example.org/onto/prop/google_container_cluster_membership">
    <rdfs:label>membership</rdfs:label>
    <rdfs:comment>Full resource name of the registered fleet membership of the cluster.</rdfs:comment>
    <rdfs:domain rdf:resource="http://example.org/onto/class/google_container_cluster"/>
    <rdfs:range rdf:resource="http://www.w3.org/2001/XMLSchema#string"/>
  </owl:DatatypeProperty>
  <owl:DatatypeProperty rdf:about="http://example.org/onto/prop/google_container_cluster_membership_id">
    <rdfs:label>membership_id</rdfs:label>
    <rdfs:comment>Short name of the fleet membership, for example "member-1".</rdfs:comment>
    <rdfs:domain rdf:resource="http://example.org/onto/class/google_container_cluster"/>
    <rdfs:range rdf:resource="http://www.w3.org/2001/XMLSchema#string"/>
  </owl:DatatypeProperty>
  <owl:DatatypeProperty rdf:about="http://example.org/onto/prop/google_container_cluster_membership_location">
    <rdfs:label>membership_location</rdfs:label>
    <rdfs:comment>Location of the fleet membership, for example "us-central1".</rdfs:comment>
    <rdfs:domain rdf:resource="http://example.org/onto/class/google_container_cluster"/>
    <rdfs:range rdf:resource="http://www.w3.org/2001/XMLSchema#string"/>
  </owl:DatatypeProperty>
  <owl:DatatypeProperty rdf:about="http://example.org/onto/prop/google_container_cluster_pre_registered">
    <rdfs:label>pre_registered</rdfs:label>
    <rdfs:comment>Whether the cluster has been registered via the fleet API.</rdfs:comment>
    <rdfs:domain rdf:resource="http://example.org/onto/class/google_container_cluster"/>
    <rdfs:range rdf:resource="http://www.w3.org/2001/XMLSchema#string"/>
  </owl:DatatypeProperty>
  <owl:DatatypeProperty rdf:about="http://example.org/onto/prop/google_container_cluster_project">
    <rdfs:label>project</rdfs:label>
    <rdfs:comment>The Fleet host project of the cluster.</rdfs:comment>
    <rdfs:domain rdf:resource="http://example.org/onto/class/google_container_cluster"/>
    <rdfs:range rdf:resource="http://www.w3.org/2001/XMLSchema#string"/>
  </owl:DatatypeProperty>
  <owl:DatatypeProperty rdf:about="http://example.org/onto/prop/google_container_cluster_channel">
    <rdfs:label>channel</rdfs:label>
    <rdfs:comment>The Gateway API release channel to use for Gateway API.</rdfs:comment>
    <rdfs:domain rdf:resource="http://example.org/onto/class/google_container_cluster"/>
    <rdfs:range rdf:resource="http://www.w3.org/2001/XMLSchema#string"/>
  </owl:DatatypeProperty>
  <owl:DatatypeProperty rdf:about="http://example.org/onto/prop/google_container_cluster_patch_mode">
    <rdfs:label>patch_mode</rdfs:label>
    <rdfs:comment>The selected auto-upgrade patch type. Accepted values are:
* ACCELERATED: Upgrades to the latest available patch version in a given minor and release channel.</rdfs:comment>
    <rdfs:domain rdf:resource="http://example.org/onto/class/google_container_cluster"/>
    <rdfs:range rdf:resource="http://www.w3.org/2001/XMLSchema#string"/>
  </owl:DatatypeProperty>
  <owl:DatatypeProperty rdf:about="http://example.org/onto/prop/google_container_cluster_enabled">
    <rdfs:label>enabled</rdfs:label>
    <rdfs:comment>Whether to enable the Identity Service component.</rdfs:comment>
    <rdfs:domain rdf:resource="http://example.org/onto/class/google_container_cluster"/>
    <rdfs:range rdf:resource="http://www.w3.org/2001/XMLSchema#string"/>
  </owl:DatatypeProperty>
  <owl:DatatypeProperty rdf:about="http://example.org/onto/prop/google_container_cluster_cluster_ipv4_cidr_block">
    <rdfs:label>cluster_ipv4_cidr_block</rdfs:label>
    <rdfs:comment>The IP address range for the cluster pod IPs. Set to blank to have a range chosen with the default size. Set to /netmask (e.g. /14) to have a range chosen with a specific netmask. Set to a CIDR notation (e.g. 10.96.0.0/14) from the RFC-1918 private networks (e.g. 10.0.0.0/8, 172.16.0.0/12, 192.168.0.0/16) to pick a specific range to use.</rdfs:comment>
    <rdfs:domain rdf:resource="http://example.org/onto/class/google_container_cluster"/>
    <rdfs:range rdf:resource="http://www.w3.org/2001/XMLSchema#string"/>
  </owl:DatatypeProperty>
  <owl:DatatypeProperty rdf:about="http://example.org/onto/prop/google_container_cluster_cluster_secondary_range_name">
    <rdfs:label>cluster_secondary_range_name</rdfs:label>
    <rdfs:comment>The name of the existing secondary range in the cluster's subnetwork to use for pod IP addresses. Alternatively, cluster_ipv4_cidr_block can be used to automatically create a GKE-managed one.</rdfs:comment>
    <rdfs:domain rdf:resource="http://example.org/onto/class/google_container_cluster"/>
    <rdfs:range rdf:resource="http://www.w3.org/2001/XMLSchema#string"/>
  </owl:DatatypeProperty>
  <owl:DatatypeProperty rdf:about="http://example.org/onto/prop/google_container_cluster_services_ipv4_cidr_block">
    <rdfs:label>services_ipv4_cidr_block</rdfs:label>
    <rdfs:comment>The IP address range of the services IPs in this cluster. Set to blank to have a range chosen with the default size. Set to /netmask (e.g. /14) to have a range chosen with a specific netmask. Set to a CIDR notation (e.g. 10.96.0.0/14) from the RFC-1918 private networks (e.g. 10.0.0.0/8, 172.16.0.0/12, 192.168.0.0/16) to pick a specific range to use.</rdfs:comment>
    <rdfs:domain rdf:resource="http://example.org/onto/class/google_container_cluster"/>
    <rdfs:range rdf:resource="http://www.w3.org/2001/XMLSchema#string"/>
  </owl:DatatypeProperty>
  <owl:DatatypeProperty rdf:about="http://example.org/onto/prop/google_container_cluster_services_secondary_range_name">
    <rdfs:label>services_secondary_range_name</rdfs:label>
    <rdfs:comment>The name of the existing secondary range in the cluster's subnetwork to use for service ClusterIPs. Alternatively, services_ipv4_cidr_block can be used to automatically create a GKE-managed one.</rdfs:comment>
    <rdfs:domain rdf:resource="http://example.org/onto/class/google_container_cluster"/>
    <rdfs:range rdf:resource="http://www.w3.org/2001/XMLSchema#string"/>
  </owl:DatatypeProperty>
  <owl:DatatypeProperty rdf:about="http://example.org/onto/prop/google_container_cluster_stack_type">
    <rdfs:label>stack_type</rdfs:label>
    <rdfs:comment>The IP Stack type of the cluster. Choose between IPV4 and IPV4_IPV6. Default type is IPV4 Only if not set</rdfs:comment>
    <rdfs:domain rdf:resource="http://example.org/onto/class/google_container_cluster"/>
    <rdfs:range rdf:resource="http://www.w3.org/2001/XMLSchema#string"/>
  </owl:DatatypeProperty>
  <owl:DatatypeProperty rdf:about="http://example.org/onto/prop/google_container_cluster_pod_ipv4_range_names">
    <rdfs:label>pod_ipv4_range_names</rdfs:label>
    <rdfs:comment>List of secondary ranges names within this subnetwork that can be used for pod IPs.</rdfs:comment>
    <rdfs:domain rdf:resource="http://example.org/onto/class/google_container_cluster"/>
    <rdfs:range rdf:resource="http://www.w3.org/2001/XMLSchema#string"/>
  </owl:DatatypeProperty>
  <owl:DatatypeProperty rdf:about="http://example.org/onto/prop/google_container_cluster_subnetwork">
    <rdfs:label>subnetwork</rdfs:label>
    <rdfs:comment>Name of the subnetwork. This can be the full path of the subnetwork or just the name.</rdfs:comment>
    <rdfs:domain rdf:resource="http://example.org/onto/class/google_container_cluster"/>
    <rdfs:range rdf:resource="http://www.w3.org/2001/XMLSchema#string"/>
  </owl:DatatypeProperty>
  <owl:DatatypeProperty rdf:about="http://example.org/onto/prop/google_container_cluster_pod_range_names">
    <rdfs:label>pod_range_names</rdfs:label>
    <rdfs:comment>Name for pod secondary ipv4 range which has the actual range defined ahead.</rdfs:comment>
    <rdfs:domain rdf:resource="http://example.org/onto/class/google_container_cluster"/>
    <rdfs:range rdf:resource="http://www.w3.org/2001/XMLSchema#string"/>
  </owl:DatatypeProperty>
  <owl:DatatypeProperty rdf:about="http://example.org/onto/prop/google_container_cluster_enabled">
    <rdfs:label>enabled</rdfs:label>
    <rdfs:comment>The flag that enables Auto IPAM on this cluster.</rdfs:comment>
    <rdfs:domain rdf:resource="http://example.org/onto/class/google_container_cluster"/>
    <rdfs:range rdf:resource="http://www.w3.org/2001/XMLSchema#string"/>
  </owl:DatatypeProperty>
  <owl:DatatypeProperty rdf:about="http://example.org/onto/prop/google_container_cluster_disabled">
    <rdfs:label>disabled</rdfs:label>
    <rdfs:domain rdf:resource="http://example.org/onto/class/google_container_cluster"/>
    <rdfs:range rdf:resource="http://www.w3.org/2001/XMLSchema#string"/>
  </owl:DatatypeProperty>
  <owl:DatatypeProperty rdf:about="http://example.org/onto/prop/google_container_cluster_enable_components">
    <rdfs:label>enable_components</rdfs:label>
    <rdfs:comment>GKE components exposing logs. Valid values include SYSTEM_COMPONENTS, APISERVER, CONTROLLER_MANAGER, KCP_CONNECTION, KCP_SSHD, KCP_HPA, SCHEDULER, and WORKLOADS.</rdfs:comment>
    <rdfs:domain rdf:resource="http://example.org/onto/class/google_container_cluster"/>
    <rdfs:range rdf:resource="http://www.w3.org/2001/XMLSchema#string"/>
  </owl:DatatypeProperty>
  <owl:DatatypeProperty rdf:about="http://example.org/onto/prop/google_container_cluster_duration">
    <rdfs:label>duration</rdfs:label>
    <rdfs:domain rdf:resource="http://example.org/onto/class/google_container_cluster"/>
    <rdfs:range rdf:resource="http://www.w3.org/2001/XMLSchema#string"/>
  </owl:DatatypeProperty>
  <owl:DatatypeProperty rdf:about="http://example.org/onto/prop/google_container_cluster_start_time">
    <rdfs:label>start_time</rdfs:label>
    <rdfs:domain rdf:resource="http://example.org/onto/class/google_container_cluster"/>
    <rdfs:range rdf:resource="http://www.w3.org/2001/XMLSchema#string"/>
  </owl:DatatypeProperty>
  <owl:DatatypeProperty rdf:about="http://example.org/onto/prop/google_container_cluster_end_time">
    <rdfs:label>end_time</rdfs:label>
    <rdfs:domain rdf:resource="http://example.org/onto/class/google_container_cluster"/>
    <rdfs:range rdf:resource="http://www.w3.org/2001/XMLSchema#string"/>
  </owl:DatatypeProperty>
  <owl:DatatypeProperty rdf:about="http://example.org/onto/prop/google_container_cluster_exclusion_name">
    <rdfs:label>exclusion_name</rdfs:label>
    <rdfs:domain rdf:resource="http://example.org/onto/class/google_container_cluster"/>
    <rdfs:range rdf:resource="http://www.w3.org/2001/XMLSchema#string"/>
  </owl:DatatypeProperty>
  <owl:DatatypeProperty rdf:about="http://example.org/onto/prop/google_container_cluster_start_time">
    <rdfs:label>start_time</rdfs:label>
    <rdfs:domain rdf:resource="http://example.org/onto/class/google_container_cluster"/>
    <rdfs:range rdf:resource="http://www.w3.org/2001/XMLSchema#string"/>
  </owl:DatatypeProperty>
  <owl:DatatypeProperty rdf:about="http://example.org/onto/prop/google_container_cluster_scope">
    <rdfs:label>scope</rdfs:label>
    <rdfs:comment>The scope of automatic upgrades to restrict in the exclusion window.</rdfs:comment>
    <rdfs:domain rdf:resource="http://example.org/onto/class/google_container_cluster"/>
    <rdfs:range rdf:resource="http://www.w3.org/2001/XMLSchema#string"/>
  </owl:DatatypeProperty>
  <owl:DatatypeProperty rdf:about="http://example.org/onto/prop/google_container_cluster_end_time">
    <rdfs:label>end_time</rdfs:label>
    <rdfs:domain rdf:resource="http://example.org/onto/class/google_container_cluster"/>
    <rdfs:range rdf:resource="http://www.w3.org/2001/XMLSchema#string"/>
  </owl:DatatypeProperty>
  <owl:DatatypeProperty rdf:about="http://example.org/onto/prop/google_container_cluster_recurrence">
    <rdfs:label>recurrence</rdfs:label>
    <rdfs:domain rdf:resource="http://example.org/onto/class/google_container_cluster"/>
    <rdfs:range rdf:resource="http://www.w3.org/2001/XMLSchema#string"/>
  </owl:DatatypeProperty>
  <owl:DatatypeProperty rdf:about="http://example.org/onto/prop/google_container_cluster_start_time">
    <rdfs:label>start_time</rdfs:label>
    <rdfs:domain rdf:resource="http://example.org/onto/class/google_container_cluster"/>
    <rdfs:range rdf:resource="http://www.w3.org/2001/XMLSchema#string"/>
  </owl:DatatypeProperty>
  <owl:DatatypeProperty rdf:about="http://example.org/onto/prop/google_container_cluster_client_certificate">
    <rdfs:label>client_certificate</rdfs:label>
    <rdfs:comment>Base64 encoded public certificate used by clients to authenticate to the cluster endpoint.</rdfs:comment>
    <rdfs:domain rdf:resource="http://example.org/onto/class/google_container_cluster"/>
    <rdfs:range rdf:resource="http://www.w3.org/2001/XMLSchema#string"/>
  </owl:DatatypeProperty>
  <owl:DatatypeProperty rdf:about="http://example.org/onto/prop/google_container_cluster_client_key">
    <rdfs:label>client_key</rdfs:label>
    <rdfs:comment>Base64 encoded private key used by clients to authenticate to the cluster endpoint.</rdfs:comment>
    <rdfs:domain rdf:resource="http://example.org/onto/class/google_container_cluster"/>
    <rdfs:range rdf:resource="http://www.w3.org/2001/XMLSchema#string"/>
  </owl:DatatypeProperty>
  <owl:DatatypeProperty rdf:about="http://example.org/onto/prop/google_container_cluster_cluster_ca_certificate">
    <rdfs:label>cluster_ca_certificate</rdfs:label>
    <rdfs:comment>Base64 encoded public certificate that is the root of trust for the cluster.</rdfs:comment>
    <rdfs:domain rdf:resource="http://example.org/onto/class/google_container_cluster"/>
    <rdfs:range rdf:resource="http://www.w3.org/2001/XMLSchema#string"/>
  </owl:DatatypeProperty>
  <owl:DatatypeProperty rdf:about="http://example.org/onto/prop/google_container_cluster_issue_client_certificate">
    <rdfs:label>issue_client_certificate</rdfs:label>
    <rdfs:comment>Whether client certificate authorization is enabled for this cluster.</rdfs:comment>
    <rdfs:domain rdf:resource="http://example.org/onto/class/google_container_cluster"/>
    <rdfs:range rdf:resource="http://www.w3.org/2001/XMLSchema#string"/>
  </owl:DatatypeProperty>
  <owl:DatatypeProperty rdf:about="http://example.org/onto/prop/google_container_cluster_gcp_public_cidrs_access_enabled">
    <rdfs:label>gcp_public_cidrs_access_enabled</rdfs:label>
    <rdfs:comment>Whether Kubernetes master is accessible via Google Compute Engine Public IPs.</rdfs:comment>
    <rdfs:domain rdf:resource="http://example.org/onto/class/google_container_cluster"/>
    <rdfs:range rdf:resource="http://www.w3.org/2001/XMLSchema#string"/>
  </owl:DatatypeProperty>
  <owl:DatatypeProperty rdf:about="http://example.org/onto/prop/google_container_cluster_private_endpoint_enforcement_enabled">
    <rdfs:label>private_endpoint_enforcement_enabled</rdfs:label>
    <rdfs:comment>Whether authorized networks is enforced on the private endpoint or not. Defaults to false.</rdfs:comment>
    <rdfs:domain rdf:resource="http://example.org/onto/class/google_container_cluster"/>
    <rdfs:range rdf:resource="http://www.w3.org/2001/XMLSchema#string"/>
  </owl:DatatypeProperty>
  <owl:DatatypeProperty rdf:about="http://example.org/onto/prop/google_container_cluster_cidr_block">
    <rdfs:label>cidr_block</rdfs:label>
    <rdfs:comment>External network that can access Kubernetes master through HTTPS. Must be specified in CIDR notation.</rdfs:comment>
    <rdfs:domain rdf:resource="http://example.org/onto/class/google_container_cluster"/>
    <rdfs:range rdf:resource="http://www.w3.org/2001/XMLSchema#string"/>
  </owl:DatatypeProperty>
  <owl:DatatypeProperty rdf:about="http://example.org/onto/prop/google_container_cluster_display_name">
    <rdfs:label>display_name</rdfs:label>
    <rdfs:comment>Field for users to identify CIDR blocks.</rdfs:comment>
    <rdfs:domain rdf:resource="http://example.org/onto/class/google_container_cluster"/>
    <rdfs:range rdf:resource="http://www.w3.org/2001/XMLSchema#string"/>
  </owl:DatatypeProperty>
  <owl:DatatypeProperty rdf:about="http://example.org/onto/prop/google_container_cluster_enable_certificates">
    <rdfs:label>enable_certificates</rdfs:label>
    <rdfs:comment>When enabled the GKE Workload Identity Certificates controller and node agent will be deployed in the cluster.</rdfs:comment>
    <rdfs:domain rdf:resource="http://example.org/onto/class/google_container_cluster"/>
    <rdfs:range rdf:resource="http://www.w3.org/2001/XMLSchema#string"/>
  </owl:DatatypeProperty>
  <owl:DatatypeProperty rdf:about="http://example.org/onto/prop/google_container_cluster_enable_components">
    <rdfs:label>enable_components</rdfs:label>
    <rdfs:comment>GKE components exposing metrics. Valid values include SYSTEM_COMPONENTS, APISERVER, SCHEDULER, CONTROLLER_MANAGER, STORAGE, HPA, POD, DAEMONSET, DEPLOYMENT, STATEFULSET, KUBELET, CADVISOR, DCGM and JOBSET.</rdfs:comment>
    <rdfs:domain rdf:resource="http://example.org/onto/class/google_container_cluster"/>
    <rdfs:range rdf:resource="http://www.w3.org/2001/XMLSchema#string"/>
  </owl:DatatypeProperty>
  <owl:DatatypeProperty rdf:about="http://example.org/onto/prop/google_container_cluster_enable_metrics">
    <rdfs:label>enable_metrics</rdfs:label>
    <rdfs:comment>Whether or not the advanced datapath metrics are enabled.</rdfs:comment>
    <rdfs:domain rdf:resource="http://example.org/onto/class/google_container_cluster"/>
    <rdfs:range rdf:resource="http://www.w3.org/2001/XMLSchema#string"/>
  </owl:DatatypeProperty>
  <owl:DatatypeProperty rdf:about="http://example.org/onto/prop/google_container_cluster_enable_relay">
    <rdfs:label>enable_relay</rdfs:label>
    <rdfs:comment>Whether or not Relay is enabled.</rdfs:comment>
    <rdfs:domain rdf:resource="http://example.org/onto/class/google_container_cluster"/>
    <rdfs:range rdf:resource="http://www.w3.org/2001/XMLSchema#string"/>
  </owl:DatatypeProperty>
  <owl:DatatypeProperty rdf:about="http://example.org/onto/prop/google_container_cluster_enabled">
    <rdfs:label>enabled</rdfs:label>
    <rdfs:comment>Whether or not the managed collection is enabled.</rdfs:comment>
    <rdfs:domain rdf:resource="http://example.org/onto/class/google_container_cluster"/>
    <rdfs:range rdf:resource="http://www.w3.org/2001/XMLSchema#string"/>
  </owl:DatatypeProperty>
  <owl:DatatypeProperty rdf:about="http://example.org/onto/prop/google_container_cluster_scope">
    <rdfs:label>scope</rdfs:label>
    <rdfs:comment>The scope of auto-monitoring.</rdfs:comment>
    <rdfs:domain rdf:resource="http://example.org/onto/class/google_container_cluster"/>
    <rdfs:range rdf:resource="http://www.w3.org/2001/XMLSchema#string"/>
  </owl:DatatypeProperty>
  <owl:DatatypeProperty rdf:about="http://example.org/onto/prop/google_container_cluster_total_egress_bandwidth_tier">
    <rdfs:label>total_egress_bandwidth_tier</rdfs:label>
    <rdfs:comment>Specifies the total network bandwidth tier for NodePools in the cluster.</rdfs:comment>
    <rdfs:domain rdf:resource="http://example.org/onto/class/google_container_cluster"/>
    <rdfs:range rdf:resource="http://www.w3.org/2001/XMLSchema#string"/>
  </owl:DatatypeProperty>
  <owl:DatatypeProperty rdf:about="http://example.org/onto/prop/google_container_cluster_enabled">
    <rdfs:label>enabled</rdfs:label>
    <rdfs:comment>Whether network policy is enabled on the cluster.</rdfs:comment>
    <rdfs:domain rdf:resource="http://example.org/onto/class/google_container_cluster"/>
    <rdfs:range rdf:resource="http://www.w3.org/2001/XMLSchema#string"/>
  </owl:DatatypeProperty>
  <owl:DatatypeProperty rdf:about="http://example.org/onto/prop/google_container_cluster_provider">
    <rdfs:label>provider</rdfs:label>
    <rdfs:comment>The selected network policy provider.</rdfs:comment>
    <rdfs:domain rdf:resource="http://example.org/onto/class/google_container_cluster"/>
    <rdfs:range rdf:resource="http://www.w3.org/2001/XMLSchema#string"/>
  </owl:DatatypeProperty>
  <owl:DatatypeProperty rdf:about="http://example.org/onto/prop/google_container_cluster_boot_disk_kms_key">
    <rdfs:label>boot_disk_kms_key</rdfs:label>
    <rdfs:comment>The Customer Managed Encryption Key used to encrypt the boot disk attached to each node in the node pool.</rdfs:comment>
    <rdfs:domain rdf:resource="http://example.org/onto/class/google_container_cluster"/>
    <rdfs:range rdf:resource="http://www.w3.org/2001/XMLSchema#string"/>
  </owl:DatatypeProperty>
  <owl:DatatypeProperty rdf:about="http://example.org/onto/prop/google_container_cluster_disk_size_gb">
    <rdfs:label>disk_size_gb</rdfs:label>
    <rdfs:comment>Size of the disk attached to each node, specified in GB. The smallest allowed disk size is 10GB.</rdfs:comment>
    <rdfs:domain rdf:resource="http://example.org/onto/class/google_container_cluster"/>
    <rdfs:range rdf:resource="http://www.w3.org/2001/XMLSchema#string"/>
  </owl:DatatypeProperty>
  <owl:DatatypeProperty rdf:about="http://example.org/onto/prop/google_container_cluster_disk_type">
    <rdfs:label>disk_type</rdfs:label>
    <rdfs:comment>Type of the disk attached to each node. Such as pd-standard, pd-balanced or pd-ssd</rdfs:comment>
    <rdfs:domain rdf:resource="http://example.org/onto/class/google_container_cluster"/>
    <rdfs:range rdf:resource="http://www.w3.org/2001/XMLSchema#string"/>
  </owl:DatatypeProperty>
  <owl:DatatypeProperty rdf:about="http://example.org/onto/prop/google_container_cluster_effective_taints">
    <rdfs:label>effective_taints</rdfs:label>
    <rdfs:comment>List of kubernetes taints applied to each node.</rdfs:comment>
    <rdfs:domain rdf:resource="http://example.org/onto/class/google_container_cluster"/>
    <rdfs:range rdf:resource="http://www.w3.org/2001/XMLSchema#string"/>
  </owl:DatatypeProperty>
  <owl:DatatypeProperty rdf:about="http://example.org/onto/prop/google_container_cluster_enable_confidential_storage">
    <rdfs:label>enable_confidential_storage</rdfs:label>
    <rdfs:comment>If enabled boot disks are configured with confidential mode.</rdfs:comment>
    <rdfs:domain rdf:resource="http://example.org/onto/class/google_container_cluster"/>
    <rdfs:range rdf:resource="http://www.w3.org/2001/XMLSchema#string"/>
  </owl:DatatypeProperty>
  <owl:DatatypeProperty rdf:about="http://example.org/onto/prop/google_container_cluster_flex_start">
    <rdfs:label>flex_start</rdfs:label>
    <rdfs:comment>Enables Flex Start provisioning model for the node pool</rdfs:comment>
    <rdfs:domain rdf:resource="http://example.org/onto/class/google_container_cluster"/>
    <rdfs:range rdf:resource="http://www.w3.org/2001/XMLSchema#string"/>
  </owl:DatatypeProperty>
  <owl:DatatypeProperty rdf:about="http://example.org/onto/prop/google_container_cluster_image_type">
    <rdfs:label>image_type</rdfs:label>
    <rdfs:comment>The image type to use for this node. Note that for a given image type, the latest version of it will be used.</rdfs:comment>
    <rdfs:domain rdf:resource="http://example.org/onto/class/google_container_cluster"/>
    <rdfs:range rdf:resource="http://www.w3.org/2001/XMLSchema#string"/>
  </owl:DatatypeProperty>
  <owl:DatatypeProperty rdf:about="http://example.org/onto/prop/google_container_cluster_labels">
    <rdfs:label>labels</rdfs:label>
    <rdfs:comment>The map of Kubernetes labels (key/value pairs) to be applied to each node. These will added in addition to any default label(s) that Kubernetes may apply to the node.</rdfs:comment>
    <rdfs:domain rdf:resource="http://example.org/onto/class/google_container_cluster"/>
    <rdfs:range rdf:resource="http://www.w3.org/2001/XMLSchema#string"/>
  </owl:DatatypeProperty>
  <owl:DatatypeProperty rdf:about="http://example.org/onto/prop/google_container_cluster_local_ssd_count">
    <rdfs:label>local_ssd_count</rdfs:label>
    <rdfs:comment>The number of local SSD disks to be attached to the node.</rdfs:comment>
    <rdfs:domain rdf:resource="http://example.org/onto/class/google_container_cluster"/>
    <rdfs:range rdf:resource="http://www.w3.org/2001/XMLSchema#string"/>
  </owl:DatatypeProperty>
  <owl:DatatypeProperty rdf:about="http://example.org/onto/prop/google_container_cluster_local_ssd_encryption_mode">
    <rdfs:label>local_ssd_encryption_mode</rdfs:label>
    <rdfs:comment>LocalSsdEncryptionMode specified the method used for encrypting the local SSDs attached to the node.</rdfs:comment>
    <rdfs:domain rdf:resource="http://example.org/onto/class/google_container_cluster"/>
    <rdfs:range rdf:resource="http://www.w3.org/2001/XMLSchema#string"/>
  </owl:DatatypeProperty>
  <owl:DatatypeProperty rdf:about="http://example.org/onto/prop/google_container_cluster_logging_variant">
    <rdfs:label>logging_variant</rdfs:label>
    <rdfs:comment>Type of logging agent that is used as the default value for node pools in the cluster. Valid values include DEFAULT and MAX_THROUGHPUT.</rdfs:comment>
    <rdfs:domain rdf:resource="http://example.org/onto/class/google_container_cluster"/>
    <rdfs:range rdf:resource="http://www.w3.org/2001/XMLSchema#string"/>
  </owl:DatatypeProperty>
  <owl:DatatypeProperty rdf:about="http://example.org/onto/prop/google_container_cluster_machine_type">
    <rdfs:label>machine_type</rdfs:label>
    <rdfs:comment>The name of a Google Compute Engine machine type.</rdfs:comment>
    <rdfs:domain rdf:resource="http://example.org/onto/class/google_container_cluster"/>
    <rdfs:range rdf:resource="http://www.w3.org/2001/XMLSchema#string"/>
  </owl:DatatypeProperty>
  <owl:DatatypeProperty rdf:about="http://example.org/onto/prop/google_container_cluster_max_run_duration">
    <rdfs:label>max_run_duration</rdfs:label>
    <rdfs:comment>The runtime of each node in the node pool in seconds, terminated by 's'. Example: "3600s".</rdfs:comment>
    <rdfs:domain rdf:resource="http://example.org/onto/class/google_container_cluster"/>
    <rdfs:range rdf:resource="http://www.w3.org/2001/XMLSchema#string"/>
  </owl:DatatypeProperty>
  <owl:DatatypeProperty rdf:about="http://example.org/onto/prop/google_container_cluster_metadata">
    <rdfs:label>metadata</rdfs:label>
    <rdfs:comment>The metadata key/value pairs assigned to instances in the cluster.</rdfs:comment>
    <rdfs:domain rdf:resource="http://example.org/onto/class/google_container_cluster"/>
    <rdfs:range rdf:resource="http://www.w3.org/2001/XMLSchema#string"/>
  </owl:DatatypeProperty>
  <owl:DatatypeProperty rdf:about="http://example.org/onto/prop/google_container_cluster_min_cpu_platform">
    <rdfs:label>min_cpu_platform</rdfs:label>
    <rdfs:comment>Minimum CPU platform to be used by this instance. The instance may be scheduled on the specified or newer CPU platform.</rdfs:comment>
    <rdfs:domain rdf:resource="http://example.org/onto/class/google_container_cluster"/>
    <rdfs:range rdf:resource="http://www.w3.org/2001/XMLSchema#string"/>
  </owl:DatatypeProperty>
  <owl:DatatypeProperty rdf:about="http://example.org/onto/prop/google_container_cluster_node_group">
    <rdfs:label>node_group</rdfs:label>
    <rdfs:comment>Setting this field will assign instances of this pool to run on the specified node group. This is useful for running workloads on sole tenant nodes.</rdfs:comment>
    <rdfs:domain rdf:resource="http://example.org/onto/class/google_container_cluster"/>
    <rdfs:range rdf:resource="http://www.w3.org/2001/XMLSchema#string"/>
  </owl:DatatypeProperty>
  <owl:DatatypeProperty rdf:about="http://example.org/onto/prop/google_container_cluster_oauth_scopes">
    <rdfs:label>oauth_scopes</rdfs:label>
    <rdfs:comment>The set of Google API scopes to be made available on all of the node VMs.</rdfs:comment>
    <rdfs:domain rdf:resource="http://example.org/onto/class/google_container_cluster"/>
    <rdfs:range rdf:resource="http://www.w3.org/2001/XMLSchema#string"/>
  </owl:DatatypeProperty>
  <owl:DatatypeProperty rdf:about="http://example.org/onto/prop/google_container_cluster_preemptible">
    <rdfs:label>preemptible</rdfs:label>
    <rdfs:comment>Whether the nodes are created as preemptible VM instances.</rdfs:comment>
    <rdfs:domain rdf:resource="http://example.org/onto/class/google_container_cluster"/>
    <rdfs:range rdf:resource="http://www.w3.org/2001/XMLSchema#string"/>
  </owl:DatatypeProperty>
  <owl:DatatypeProperty rdf:about="http://example.org/onto/prop/google_container_cluster_resource_labels">
    <rdfs:label>resource_labels</rdfs:label>
    <rdfs:comment>The GCE resource labels (a map of key/value pairs) to be applied to the node pool.</rdfs:comment>
    <rdfs:domain rdf:resource="http://example.org/onto/class/google_container_cluster"/>
    <rdfs:range rdf:resource="http://www.w3.org/2001/XMLSchema#string"/>
  </owl:DatatypeProperty>
  <owl:DatatypeProperty rdf:about="http://example.org/onto/prop/google_container_cluster_resource_manager_tags">
    <rdfs:label>resource_manager_tags</rdfs:label>
    <rdfs:comment>A map of resource manager tags. Resource manager tag keys and values have the same definition as resource manager tags. Keys must be in the format tagKeys/{tag_key_id}, and values are in the format tagValues/456. The field is ignored (both PUT & PATCH) when empty.</rdfs:comment>
    <rdfs:domain rdf:resource="http://example.org/onto/class/google_container_cluster"/>
    <rdfs:range rdf:resource="http://www.w3.org/2001/XMLSchema#string"/>
  </owl:DatatypeProperty>
  <owl:DatatypeProperty rdf:about="http://example.org/onto/prop/google_container_cluster_service_account">
    <rdfs:label>service_account</rdfs:label>
    <rdfs:comment>The Google Cloud Platform Service Account to be used by the node VMs.</rdfs:comment>
    <rdfs:domain rdf:resource="http://example.org/onto/class/google_container_cluster"/>
    <rdfs:range rdf:resource="http://www.w3.org/2001/XMLSchema#string"/>
  </owl:DatatypeProperty>
  <owl:DatatypeProperty rdf:about="http://example.org/onto/prop/google_container_cluster_spot">
    <rdfs:label>spot</rdfs:label>
    <rdfs:comment>Whether the nodes are created as spot VM instances.</rdfs:comment>
    <rdfs:domain rdf:resource="http://example.org/onto/class/google_container_cluster"/>
    <rdfs:range rdf:resource="http://www.w3.org/2001/XMLSchema#string"/>
  </owl:DatatypeProperty>
  <owl:DatatypeProperty rdf:about="http://example.org/onto/prop/google_container_cluster_storage_pools">
    <rdfs:label>storage_pools</rdfs:label>
    <rdfs:comment>The list of Storage Pools where boot disks are provisioned.</rdfs:comment>
    <rdfs:domain rdf:resource="http://example.org/onto/class/google_container_cluster"/>
    <rdfs:range rdf:resource="http://www.w3.org/2001/XMLSchema#string"/>
  </owl:DatatypeProperty>
  <owl:DatatypeProperty rdf:about="http://example.org/onto/prop/google_container_cluster_tags">
    <rdfs:label>tags</rdfs:label>
    <rdfs:comment>The list of instance tags applied to all nodes.</rdfs:comment>
    <rdfs:domain rdf:resource="http://example.org/onto/class/google_container_cluster"/>
    <rdfs:range rdf:resource="http://www.w3.org/2001/XMLSchema#string"/>
  </owl:DatatypeProperty>
  <owl:DatatypeProperty rdf:about="http://example.org/onto/prop/google_container_cluster_enable_nested_virtualization">
    <rdfs:label>enable_nested_virtualization</rdfs:label>
    <rdfs:comment>Whether the node should have nested virtualization enabled.</rdfs:comment>
    <rdfs:domain rdf:resource="http://example.org/onto/class/google_container_cluster"/>
    <rdfs:range rdf:resource="http://www.w3.org/2001/XMLSchema#string"/>
  </owl:DatatypeProperty>
  <owl:DatatypeProperty rdf:about="http://example.org/onto/prop/google_container_cluster_performance_monitoring_unit">
    <rdfs:label>performance_monitoring_unit</rdfs:label>
    <rdfs:comment>Level of Performance Monitoring Unit (PMU) requested. If unset, no access to the PMU is assumed.</rdfs:comment>
    <rdfs:domain rdf:resource="http://example.org/onto/class/google_container_cluster"/>
    <rdfs:range rdf:resource="http://www.w3.org/2001/XMLSchema#string"/>
  </owl:DatatypeProperty>
  <owl:DatatypeProperty rdf:about="http://example.org/onto/prop/google_container_cluster_threads_per_core">
    <rdfs:label>threads_per_core</rdfs:label>
    <rdfs:comment>The number of threads per physical core. To disable simultaneous multithreading (SMT) set this to 1. If unset, the maximum number of threads supported per core by the underlying processor is assumed.</rdfs:comment>
    <rdfs:domain rdf:resource="http://example.org/onto/class/google_container_cluster"/>
    <rdfs:range rdf:resource="http://www.w3.org/2001/XMLSchema#string"/>
  </owl:DatatypeProperty>
  <owl:DatatypeProperty rdf:about="http://example.org/onto/prop/google_container_cluster_disk_type">
    <rdfs:label>disk_type</rdfs:label>
    <rdfs:comment>Type of the disk attached to each node. Such as pd-standard, pd-balanced or pd-ssd</rdfs:comment>
    <rdfs:domain rdf:resource="http://example.org/onto/class/google_container_cluster"/>
    <rdfs:range rdf:resource="http://www.w3.org/2001/XMLSchema#string"/>
  </owl:DatatypeProperty>
  <owl:DatatypeProperty rdf:about="http://example.org/onto/prop/google_container_cluster_provisioned_iops">
    <rdfs:label>provisioned_iops</rdfs:label>
    <rdfs:comment>Configured IOPs provisioning. Only valid with disk type hyperdisk-balanced.</rdfs:comment>
    <rdfs:domain rdf:resource="http://example.org/onto/class/google_container_cluster"/>
    <rdfs:range rdf:resource="http://www.w3.org/2001/XMLSchema#string"/>
  </owl:DatatypeProperty>
  <owl:DatatypeProperty rdf:about="http://example.org/onto/prop/google_container_cluster_provisioned_throughput">
    <rdfs:label>provisioned_throughput</rdfs:label>
    <rdfs:comment>Configured throughput provisioning. Only valid with disk type hyperdisk-balanced.</rdfs:comment>
    <rdfs:domain rdf:resource="http://example.org/onto/class/google_container_cluster"/>
    <rdfs:range rdf:resource="http://www.w3.org/2001/XMLSchema#string"/>
  </owl:DatatypeProperty>
  <owl:DatatypeProperty rdf:about="http://example.org/onto/prop/google_container_cluster_size_gb">
    <rdfs:label>size_gb</rdfs:label>
    <rdfs:comment>Size of the disk attached to each node, specified in GB. The smallest allowed disk size is 10GB.</rdfs:comment>
    <rdfs:domain rdf:resource="http://example.org/onto/class/google_container_cluster"/>
    <rdfs:range rdf:resource="http://www.w3.org/2001/XMLSchema#string"/>
  </owl:DatatypeProperty>
  <owl:DatatypeProperty rdf:about="http://example.org/onto/prop/google_container_cluster_confidential_instance_type">
    <rdfs:label>confidential_instance_type</rdfs:label>
    <rdfs:comment>Defines the type of technology used by the confidential node.</rdfs:comment>
    <rdfs:domain rdf:resource="http://example.org/onto/class/google_container_cluster"/>
    <rdfs:range rdf:resource="http://www.w3.org/2001/XMLSchema#string"/>
  </owl:DatatypeProperty>
  <owl:DatatypeProperty rdf:about="http://example.org/onto/prop/google_container_cluster_enabled">
    <rdfs:label>enabled</rdfs:label>
    <rdfs:comment>Whether Confidential Nodes feature is enabled for all nodes in this pool.</rdfs:comment>
    <rdfs:domain rdf:resource="http://example.org/onto/class/google_container_cluster"/>
    <rdfs:range rdf:resource="http://www.w3.org/2001/XMLSchema#string"/>
  </owl:DatatypeProperty>
  <owl:DatatypeProperty rdf:about="http://example.org/onto/prop/google_container_cluster_enabled">
    <rdfs:label>enabled</rdfs:label>
    <rdfs:comment>Whether or not private registries are configured.</rdfs:comment>
    <rdfs:domain rdf:resource="http://example.org/onto/class/google_container_cluster"/>
    <rdfs:range rdf:resource="http://www.w3.org/2001/XMLSchema#string"/>
  </owl:DatatypeProperty>
  <owl:DatatypeProperty rdf:about="http://example.org/onto/prop/google_container_cluster_fqdns">
    <rdfs:label>fqdns</rdfs:label>
    <rdfs:comment>List of fully-qualified-domain-names. IPv4s and port specification are supported.</rdfs:comment>
    <rdfs:domain rdf:resource="http://example.org/onto/class/google_container_cluster"/>
    <rdfs:range rdf:resource="http://www.w3.org/2001/XMLSchema#string"/>
  </owl:DatatypeProperty>
  <owl:DatatypeProperty rdf:about="http://example.org/onto/prop/google_container_cluster_secret_uri">
    <rdfs:label>secret_uri</rdfs:label>
    <rdfs:comment>URI for the secret that hosts a certificate. Must be in the format 'projects/PROJECT_NUM/secrets/SECRET_NAME/versions/VERSION_OR_LATEST'.</rdfs:comment>
    <rdfs:domain rdf:resource="http://example.org/onto/class/google_container_cluster"/>
    <rdfs:range rdf:resource="http://www.w3.org/2001/XMLSchema#string"/>
  </owl:DatatypeProperty>
  <owl:DatatypeProperty rdf:about="http://example.org/onto/prop/google_container_cluster_data_cache_count">
    <rdfs:label>data_cache_count</rdfs:label>
    <rdfs:comment>Number of local SSDs to be utilized for GKE Data Cache. Uses NVMe interfaces.</rdfs:comment>
    <rdfs:domain rdf:resource="http://example.org/onto/class/google_container_cluster"/>
    <rdfs:range rdf:resource="http://www.w3.org/2001/XMLSchema#string"/>
  </owl:DatatypeProperty>
  <owl:DatatypeProperty rdf:about="http://example.org/onto/prop/google_container_cluster_local_ssd_count">
    <rdfs:label>local_ssd_count</rdfs:label>
    <rdfs:comment>Number of local SSDs to use to back ephemeral storage. Uses NVMe interfaces. Each local SSD must be 375 or 3000 GB in size, and all local SSDs must share the same size.</rdfs:comment>
    <rdfs:domain rdf:resource="http://example.org/onto/class/google_container_cluster"/>
    <rdfs:range rdf:resource="http://www.w3.org/2001/XMLSchema#string"/>
  </owl:DatatypeProperty>
  <owl:DatatypeProperty rdf:about="http://example.org/onto/prop/google_container_cluster_enabled">
    <rdfs:label>enabled</rdfs:label>
    <rdfs:comment>Whether or not NCCL Fast Socket is enabled</rdfs:comment>
    <rdfs:domain rdf:resource="http://example.org/onto/class/google_container_cluster"/>
    <rdfs:range rdf:resource="http://www.w3.org/2001/XMLSchema#string"/>
  </owl:DatatypeProperty>
  <owl:DatatypeProperty rdf:about="http://example.org/onto/prop/google_container_cluster_enabled">
    <rdfs:label>enabled</rdfs:label>
    <rdfs:comment>Whether or not GCFS is enabled</rdfs:comment>
    <rdfs:domain rdf:resource="http://example.org/onto/class/google_container_cluster"/>
    <rdfs:range rdf:resource="http://www.w3.org/2001/XMLSchema#string"/>
  </owl:DatatypeProperty>
  <owl:DatatypeProperty rdf:about="http://example.org/onto/prop/google_container_cluster_count">
    <rdfs:label>count</rdfs:label>
    <rdfs:comment>The number of the accelerator cards exposed to an instance.</rdfs:comment>
    <rdfs:domain rdf:resource="http://example.org/onto/class/google_container_cluster"/>
    <rdfs:range rdf:resource="http://www.w3.org/2001/XMLSchema#string"/>
  </owl:DatatypeProperty>
  <owl:DatatypeProperty rdf:about="http://example.org/onto/prop/google_container_cluster_gpu_partition_size">
    <rdfs:label>gpu_partition_size</rdfs:label>
    <rdfs:comment>Size of partitions to create on the GPU. Valid values are described in the NVIDIA mig user guide (https://docs.nvidia.com/datacenter/tesla/mig-user-guide/#partitioning)</rdfs:comment>
    <rdfs:domain rdf:resource="http://example.org/onto/class/google_container_cluster"/>
    <rdfs:range rdf:resource="http://www.w3.org/2001/XMLSchema#string"/>
  </owl:DatatypeProperty>
  <owl:DatatypeProperty rdf:about="http://example.org/onto/prop/google_container_cluster_type">
    <rdfs:label>type</rdfs:label>
    <rdfs:comment>The accelerator type resource name.</rdfs:comment>
    <rdfs:domain rdf:resource="http://example.org/onto/class/google_container_cluster"/>
    <rdfs:range rdf:resource="http://www.w3.org/2001/XMLSchema#string"/>
  </owl:DatatypeProperty>
  <owl:DatatypeProperty rdf:about="http://example.org/onto/prop/google_container_cluster_gpu_driver_version">
    <rdfs:label>gpu_driver_version</rdfs:label>
    <rdfs:comment>Mode for how the GPU driver is installed.</rdfs:comment>
    <rdfs:domain rdf:resource="http://example.org/onto/class/google_container_cluster"/>
    <rdfs:range rdf:resource="http://www.w3.org/2001/XMLSchema#string"/>
  </owl:DatatypeProperty>
  <owl:DatatypeProperty rdf:about="http://example.org/onto/prop/google_container_cluster_gpu_sharing_strategy">
    <rdfs:label>gpu_sharing_strategy</rdfs:label>
    <rdfs:comment>The type of GPU sharing strategy to enable on the GPU node. Possible values are described in the API package (https://pkg.go.dev/google.golang.org/api/container/v1#GPUSharingConfig)</rdfs:comment>
    <rdfs:domain rdf:resource="http://example.org/onto/class/google_container_cluster"/>
    <rdfs:range rdf:resource="http://www.w3.org/2001/XMLSchema#string"/>
  </owl:DatatypeProperty>
  <owl:DatatypeProperty rdf:about="http://example.org/onto/prop/google_container_cluster_max_shared_clients_per_gpu">
    <rdfs:label>max_shared_clients_per_gpu</rdfs:label>
    <rdfs:comment>The maximum number of containers that can share a GPU.</rdfs:comment>
    <rdfs:domain rdf:resource="http://example.org/onto/class/google_container_cluster"/>
    <rdfs:range rdf:resource="http://www.w3.org/2001/XMLSchema#string"/>
  </owl:DatatypeProperty>
  <owl:DatatypeProperty rdf:about="http://example.org/onto/prop/google_container_cluster_enabled">
    <rdfs:label>enabled</rdfs:label>
    <rdfs:comment>Whether or not gvnic is enabled</rdfs:comment>
    <rdfs:domain rdf:resource="http://example.org/onto/class/google_container_cluster"/>
    <rdfs:range rdf:resource="http://www.w3.org/2001/XMLSchema#string"/>
  </owl:DatatypeProperty>
  <owl:DatatypeProperty rdf:about="http://example.org/onto/prop/google_container_cluster_maintenance_interval">
    <rdfs:label>maintenance_interval</rdfs:label>
    <rdfs:comment>.</rdfs:comment>
    <rdfs:domain rdf:resource="http://example.org/onto/class/google_container_cluster"/>
    <rdfs:range rdf:resource="http://www.w3.org/2001/XMLSchema#string"/>
  </owl:DatatypeProperty>
  <owl:DatatypeProperty rdf:about="http://example.org/onto/prop/google_container_cluster_allowed_unsafe_sysctls">
    <rdfs:label>allowed_unsafe_sysctls</rdfs:label>
    <rdfs:comment>Defines a comma-separated allowlist of unsafe sysctls or sysctl patterns which can be set on the Pods.</rdfs:comment>
    <rdfs:domain rdf:resource="http://example.org/onto/class/google_container_cluster"/>
    <rdfs:range rdf:resource="http://www.w3.org/2001/XMLSchema#string"/>
  </owl:DatatypeProperty>
  <owl:DatatypeProperty rdf:about="http://example.org/onto/prop/google_container_cluster_container_log_max_files">
    <rdfs:label>container_log_max_files</rdfs:label>
    <rdfs:comment>Defines the maximum number of container log files that can be present for a container.</rdfs:comment>
    <rdfs:domain rdf:resource="http://example.org/onto/class/google_container_cluster"/>
    <rdfs:range rdf:resource="http://www.w3.org/2001/XMLSchema#string"/>
  </owl:DatatypeProperty>
  <owl:DatatypeProperty rdf:about="http://example.org/onto/prop/google_container_cluster_container_log_max_size">
    <rdfs:label>container_log_max_size</rdfs:label>
    <rdfs:comment>Defines the maximum size of the container log file before it is rotated.</rdfs:comment>
    <rdfs:domain rdf:resource="http://example.org/onto/class/google_container_cluster"/>
    <rdfs:range rdf:resource="http://www.w3.org/2001/XMLSchema#string"/>
  </owl:DatatypeProperty>
  <owl:DatatypeProperty rdf:about="http://example.org/onto/prop/google_container_cluster_cpu_cfs_quota">
    <rdfs:label>cpu_cfs_quota</rdfs:label>
    <rdfs:comment>Enable CPU CFS quota enforcement for containers that specify CPU limits.</rdfs:comment>
    <rdfs:domain rdf:resource="http://example.org/onto/class/google_container_cluster"/>
    <rdfs:range rdf:resource="http://www.w3.org/2001/XMLSchema#string"/>
  </owl:DatatypeProperty>
  <owl:DatatypeProperty rdf:about="http://example.org/onto/prop/google_container_cluster_cpu_cfs_quota_period">
    <rdfs:label>cpu_cfs_quota_period</rdfs:label>
    <rdfs:comment>Set the CPU CFS quota period value 'cpu.cfs_period_us'.</rdfs:comment>
    <rdfs:domain rdf:resource="http://example.org/onto/class/google_container_cluster"/>
    <rdfs:range rdf:resource="http://www.w3.org/2001/XMLSchema#string"/>
  </owl:DatatypeProperty>
  <owl:DatatypeProperty rdf:about="http://example.org/onto/prop/google_container_cluster_cpu_manager_policy">
    <rdfs:label>cpu_manager_policy</rdfs:label>
    <rdfs:comment>Control the CPU management policy on the node.</rdfs:comment>
    <rdfs:domain rdf:resource="http://example.org/onto/class/google_container_cluster"/>
    <rdfs:range rdf:resource="http://www.w3.org/2001/XMLSchema#string"/>
  </owl:DatatypeProperty>
  <owl:DatatypeProperty rdf:about="http://example.org/onto/prop/google_container_cluster_eviction_max_pod_grace_period_seconds">
    <rdfs:label>eviction_max_pod_grace_period_seconds</rdfs:label>
    <rdfs:comment>Defines the maximum allowed grace period (in seconds) to use when terminating pods in response to a soft eviction threshold being met.</rdfs:comment>
    <rdfs:domain rdf:resource="http://example.org/onto/class/google_container_cluster"/>
    <rdfs:range rdf:resource="http://www.w3.org/2001/XMLSchema#string"/>
  </owl:DatatypeProperty>
  <owl:DatatypeProperty rdf:about="http://example.org/onto/prop/google_container_cluster_image_gc_high_threshold_percent">
    <rdfs:label>image_gc_high_threshold_percent</rdfs:label>
    <rdfs:comment>Defines the percent of disk usage after which image garbage collection is always run.</rdfs:comment>
    <rdfs:domain rdf:resource="http://example.org/onto/class/google_container_cluster"/>
    <rdfs:range rdf:resource="http://www.w3.org/2001/XMLSchema#string"/>
  </owl:DatatypeProperty>
  <owl:DatatypeProperty rdf:about="http://example.org/onto/prop/google_container_cluster_image_gc_low_threshold_percent">
    <rdfs:label>image_gc_low_threshold_percent</rdfs:label>
    <rdfs:comment>Defines the percent of disk usage before which image garbage collection is never run. Lowest disk usage to garbage collect to.</rdfs:comment>
    <rdfs:domain rdf:resource="http://example.org/onto/class/google_container_cluster"/>
    <rdfs:range rdf:resource="http://www.w3.org/2001/XMLSchema#string"/>
  </owl:DatatypeProperty>
  <owl:DatatypeProperty rdf:about="http://example.org/onto/prop/google_container_cluster_image_maximum_gc_age">
    <rdfs:label>image_maximum_gc_age</rdfs:label>
    <rdfs:comment>Defines the maximum age an image can be unused before it is garbage collected.</rdfs:comment>
    <rdfs:domain rdf:resource="http://example.org/onto/class/google_container_cluster"/>
    <rdfs:range rdf:resource="http://www.w3.org/2001/XMLSchema#string"/>
  </owl:DatatypeProperty>
  <owl:DatatypeProperty rdf:about="http://example.org/onto/prop/google_container_cluster_image_minimum_gc_age">
    <rdfs:label>image_minimum_gc_age</rdfs:label>
    <rdfs:comment>Defines the minimum age for an unused image before it is garbage collected.</rdfs:comment>
    <rdfs:domain rdf:resource="http://example.org/onto/class/google_container_cluster"/>
    <rdfs:range rdf:resource="http://www.w3.org/2001/XMLSchema#string"/>
  </owl:DatatypeProperty>
  <owl:DatatypeProperty rdf:about="http://example.org/onto/prop/google_container_cluster_insecure_kubelet_readonly_port_enabled">
    <rdfs:label>insecure_kubelet_readonly_port_enabled</rdfs:label>
    <rdfs:comment>Controls whether the kubelet read-only port is enabled. It is strongly recommended to set this to `FALSE`. Possible values: `TRUE`, `FALSE`.</rdfs:comment>
    <rdfs:domain rdf:resource="http://example.org/onto/class/google_container_cluster"/>
    <rdfs:range rdf:resource="http://www.w3.org/2001/XMLSchema#string"/>
  </owl:DatatypeProperty>
  <owl:DatatypeProperty rdf:about="http://example.org/onto/prop/google_container_cluster_max_parallel_image_pulls">
    <rdfs:label>max_parallel_image_pulls</rdfs:label>
    <rdfs:comment>Set the maximum number of image pulls in parallel.</rdfs:comment>
    <rdfs:domain rdf:resource="http://example.org/onto/class/google_container_cluster"/>
    <rdfs:range rdf:resource="http://www.w3.org/2001/XMLSchema#string"/>
  </owl:DatatypeProperty>
  <owl:DatatypeProperty rdf:about="http://example.org/onto/prop/google_container_cluster_pod_pids_limit">
    <rdfs:label>pod_pids_limit</rdfs:label>
    <rdfs:comment>Controls the maximum number of processes allowed to run in a pod.</rdfs:comment>
    <rdfs:domain rdf:resource="http://example.org/onto/class/google_container_cluster"/>
    <rdfs:range rdf:resource="http://www.w3.org/2001/XMLSchema#string"/>
  </owl:DatatypeProperty>
  <owl:DatatypeProperty rdf:about="http://example.org/onto/prop/google_container_cluster_single_process_oom_kill">
    <rdfs:label>single_process_oom_kill</rdfs:label>
    <rdfs:comment>Defines whether to enable single process OOM killer.</rdfs:comment>
    <rdfs:domain rdf:resource="http://example.org/onto/class/google_container_cluster"/>
    <rdfs:range rdf:resource="http://www.w3.org/2001/XMLSchema#string"/>
  </owl:DatatypeProperty>
  <owl:DatatypeProperty rdf:about="http://example.org/onto/prop/google_container_cluster_imagefs_available">
    <rdfs:label>imagefs_available</rdfs:label>
    <rdfs:comment>Defines percentage of minimum reclaim for imagefs.available.</rdfs:comment>
    <rdfs:domain rdf:resource="http://example.org/onto/class/google_container_cluster"/>
    <rdfs:range rdf:resource="http://www.w3.org/2001/XMLSchema#string"/>
  </owl:DatatypeProperty>
  <owl:DatatypeProperty rdf:about="http://example.org/onto/prop/google_container_cluster_imagefs_inodes_free">
    <rdfs:label>imagefs_inodes_free</rdfs:label>
    <rdfs:comment>Defines percentage of minimum reclaim for imagefs.inodesFree.</rdfs:comment>
    <rdfs:domain rdf:resource="http://example.org/onto/class/google_container_cluster"/>
    <rdfs:range rdf:resource="http://www.w3.org/2001/XMLSchema#string"/>
  </owl:DatatypeProperty>
  <owl:DatatypeProperty rdf:about="http://example.org/onto/prop/google_container_cluster_memory_available">
    <rdfs:label>memory_available</rdfs:label>
    <rdfs:comment>Defines percentage of minimum reclaim for memory.available.</rdfs:comment>
    <rdfs:domain rdf:resource="http://example.org/onto/class/google_container_cluster"/>
    <rdfs:range rdf:resource="http://www.w3.org/2001/XMLSchema#string"/>
  </owl:DatatypeProperty>
  <owl:DatatypeProperty rdf:about="http://example.org/onto/prop/google_container_cluster_nodefs_available">
    <rdfs:label>nodefs_available</rdfs:label>
    <rdfs:comment>Defines percentage of minimum reclaim for nodefs.available.</rdfs:comment>
    <rdfs:domain rdf:resource="http://example.org/onto/class/google_container_cluster"/>
    <rdfs:range rdf:resource="http://www.w3.org/2001/XMLSchema#string"/>
  </owl:DatatypeProperty>
  <owl:DatatypeProperty rdf:about="http://example.org/onto/prop/google_container_cluster_nodefs_inodes_free">
    <rdfs:label>nodefs_inodes_free</rdfs:label>
    <rdfs:comment>Defines percentage of minimum reclaim for nodefs.inodesFree.</rdfs:comment>
    <rdfs:domain rdf:resource="http://example.org/onto/class/google_container_cluster"/>
    <rdfs:range rdf:resource="http://www.w3.org/2001/XMLSchema#string"/>
  </owl:DatatypeProperty>
  <owl:DatatypeProperty rdf:about="http://example.org/onto/prop/google_container_cluster_pid_available">
    <rdfs:label>pid_available</rdfs:label>
    <rdfs:comment>Defines percentage of minimum reclaim for pid.available.</rdfs:comment>
    <rdfs:domain rdf:resource="http://example.org/onto/class/google_container_cluster"/>
    <rdfs:range rdf:resource="http://www.w3.org/2001/XMLSchema#string"/>
  </owl:DatatypeProperty>
  <owl:DatatypeProperty rdf:about="http://example.org/onto/prop/google_container_cluster_imagefs_available">
    <rdfs:label>imagefs_available</rdfs:label>
    <rdfs:comment>Defines percentage of soft eviction threshold for imagefs.available.</rdfs:comment>
    <rdfs:domain rdf:resource="http://example.org/onto/class/google_container_cluster"/>
    <rdfs:range rdf:resource="http://www.w3.org/2001/XMLSchema#string"/>
  </owl:DatatypeProperty>
  <owl:DatatypeProperty rdf:about="http://example.org/onto/prop/google_container_cluster_imagefs_inodes_free">
    <rdfs:label>imagefs_inodes_free</rdfs:label>
    <rdfs:comment>Defines percentage of soft eviction threshold for imagefs.inodesFree.</rdfs:comment>
    <rdfs:domain rdf:resource="http://example.org/onto/class/google_container_cluster"/>
    <rdfs:range rdf:resource="http://www.w3.org/2001/XMLSchema#string"/>
  </owl:DatatypeProperty>
  <owl:DatatypeProperty rdf:about="http://example.org/onto/prop/google_container_cluster_memory_available">
    <rdfs:label>memory_available</rdfs:label>
    <rdfs:comment>Defines quantity of soft eviction threshold for memory.available.</rdfs:comment>
    <rdfs:domain rdf:resource="http://example.org/onto/class/google_container_cluster"/>
    <rdfs:range rdf:resource="http://www.w3.org/2001/XMLSchema#string"/>
  </owl:DatatypeProperty>
  <owl:DatatypeProperty rdf:about="http://example.org/onto/prop/google_container_cluster_nodefs_available">
    <rdfs:label>nodefs_available</rdfs:label>
    <rdfs:comment>Defines percentage of soft eviction threshold for nodefs.available.</rdfs:comment>
    <rdfs:domain rdf:resource="http://example.org/onto/class/google_container_cluster"/>
    <rdfs:range rdf:resource="http://www.w3.org/2001/XMLSchema#string"/>
  </owl:DatatypeProperty>
  <owl:DatatypeProperty rdf:about="http://example.org/onto/prop/google_container_cluster_nodefs_inodes_free">
    <rdfs:label>nodefs_inodes_free</rdfs:label>
    <rdfs:comment>Defines percentage of soft eviction threshold for nodefs.inodesFree.</rdfs:comment>
    <rdfs:domain rdf:resource="http://example.org/onto/class/google_container_cluster"/>
    <rdfs:range rdf:resource="http://www.w3.org/2001/XMLSchema#string"/>
  </owl:DatatypeProperty>
  <owl:DatatypeProperty rdf:about="http://example.org/onto/prop/google_container_cluster_pid_available">
    <rdfs:label>pid_available</rdfs:label>
    <rdfs:comment>Defines percentage of soft eviction threshold for pid.available.</rdfs:comment>
    <rdfs:domain rdf:resource="http://example.org/onto/class/google_container_cluster"/>
    <rdfs:range rdf:resource="http://www.w3.org/2001/XMLSchema#string"/>
  </owl:DatatypeProperty>
  <owl:DatatypeProperty rdf:about="http://example.org/onto/prop/google_container_cluster_imagefs_available">
    <rdfs:label>imagefs_available</rdfs:label>
    <rdfs:comment>Defines grace period for the imagefs.available soft eviction threshold</rdfs:comment>
    <rdfs:domain rdf:resource="http://example.org/onto/class/google_container_cluster"/>
    <rdfs:range rdf:resource="http://www.w3.org/2001/XMLSchema#string"/>
  </owl:DatatypeProperty>
  <owl:DatatypeProperty rdf:about="http://example.org/onto/prop/google_container_cluster_imagefs_inodes_free">
    <rdfs:label>imagefs_inodes_free</rdfs:label>
    <rdfs:comment>Defines grace period for the imagefs.inodesFree soft eviction threshold.</rdfs:comment>
    <rdfs:domain rdf:resource="http://example.org/onto/class/google_container_cluster"/>
    <rdfs:range rdf:resource="http://www.w3.org/2001/XMLSchema#string"/>
  </owl:DatatypeProperty>
  <owl:DatatypeProperty rdf:about="http://example.org/onto/prop/google_container_cluster_memory_available">
    <rdfs:label>memory_available</rdfs:label>
    <rdfs:comment>Defines grace period for the memory.available soft eviction threshold.</rdfs:comment>
    <rdfs:domain rdf:resource="http://example.org/onto/class/google_container_cluster"/>
    <rdfs:range rdf:resource="http://www.w3.org/2001/XMLSchema#string"/>
  </owl:DatatypeProperty>
  <owl:DatatypeProperty rdf:about="http://example.org/onto/prop/google_container_cluster_nodefs_available">
    <rdfs:label>nodefs_available</rdfs:label>
    <rdfs:comment>Defines grace period for the nodefs.available soft eviction threshold.</rdfs:comment>
    <rdfs:domain rdf:resource="http://example.org/onto/class/google_container_cluster"/>
    <rdfs:range rdf:resource="http://www.w3.org/2001/XMLSchema#string"/>
  </owl:DatatypeProperty>
  <owl:DatatypeProperty rdf:about="http://example.org/onto/prop/google_container_cluster_nodefs_inodes_free">
    <rdfs:label>nodefs_inodes_free</rdfs:label>
    <rdfs:comment>Defines grace period for the nodefs.inodesFree soft eviction threshold.</rdfs:comment>
    <rdfs:domain rdf:resource="http://example.org/onto/class/google_container_cluster"/>
    <rdfs:range rdf:resource="http://www.w3.org/2001/XMLSchema#string"/>
  </owl:DatatypeProperty>
  <owl:DatatypeProperty rdf:about="http://example.org/onto/prop/google_container_cluster_pid_available">
    <rdfs:label>pid_available</rdfs:label>
    <rdfs:comment>Defines grace period for the pid.available soft eviction threshold.</rdfs:comment>
    <rdfs:domain rdf:resource="http://example.org/onto/class/google_container_cluster"/>
    <rdfs:range rdf:resource="http://www.w3.org/2001/XMLSchema#string"/>
  </owl:DatatypeProperty>
  <owl:DatatypeProperty rdf:about="http://example.org/onto/prop/google_container_cluster_policy">
    <rdfs:label>policy</rdfs:label>
    <rdfs:comment>The Memory Manager policy to use. This policy guides how memory and hugepages are allocated and managed for pods on the node, influencing NUMA affinity.</rdfs:comment>
    <rdfs:domain rdf:resource="http://example.org/onto/class/google_container_cluster"/>
    <rdfs:range rdf:resource="http://www.w3.org/2001/XMLSchema#string"/>
  </owl:DatatypeProperty>
  <owl:DatatypeProperty rdf:about="http://example.org/onto/prop/google_container_cluster_policy">
    <rdfs:label>policy</rdfs:label>
    <rdfs:comment>The Topology Manager policy to use. This policy dictates how resource alignment is handled on the node.</rdfs:comment>
    <rdfs:domain rdf:resource="http://example.org/onto/class/google_container_cluster"/>
    <rdfs:range rdf:resource="http://www.w3.org/2001/XMLSchema#string"/>
  </owl:DatatypeProperty>
  <owl:DatatypeProperty rdf:about="http://example.org/onto/prop/google_container_cluster_scope">
    <rdfs:label>scope</rdfs:label>
    <rdfs:comment>The Topology Manager scope, defining the granularity at which policy decisions are applied. Valid values are "container" (resources are aligned per container within a pod) or "pod" (resources are aligned for the entire pod).</rdfs:comment>
    <rdfs:domain rdf:resource="http://example.org/onto/class/google_container_cluster"/>
    <rdfs:range rdf:resource="http://www.w3.org/2001/XMLSchema#string"/>
  </owl:DatatypeProperty>
  <owl:DatatypeProperty rdf:about="http://example.org/onto/prop/google_container_cluster_cgroup_mode">
    <rdfs:label>cgroup_mode</rdfs:label>
    <rdfs:comment>cgroupMode specifies the cgroup mode to be used on the node.</rdfs:comment>
    <rdfs:domain rdf:resource="http://example.org/onto/class/google_container_cluster"/>
    <rdfs:range rdf:resource="http://www.w3.org/2001/XMLSchema#string"/>
  </owl:DatatypeProperty>
  <owl:DatatypeProperty rdf:about="http://example.org/onto/prop/google_container_cluster_sysctls">
    <rdfs:label>sysctls</rdfs:label>
    <rdfs:comment>The Linux kernel parameters to be applied to the nodes and all pods running on the nodes.</rdfs:comment>
    <rdfs:domain rdf:resource="http://example.org/onto/class/google_container_cluster"/>
    <rdfs:range rdf:resource="http://www.w3.org/2001/XMLSchema#string"/>
  </owl:DatatypeProperty>
  <owl:DatatypeProperty rdf:about="http://example.org/onto/prop/google_container_cluster_transparent_hugepage_defrag">
    <rdfs:label>transparent_hugepage_defrag</rdfs:label>
    <rdfs:comment>The Linux kernel transparent hugepage defrag setting.</rdfs:comment>
    <rdfs:domain rdf:resource="http://example.org/onto/class/google_container_cluster"/>
    <rdfs:range rdf:resource="http://www.w3.org/2001/XMLSchema#string"/>
  </owl:DatatypeProperty>
  <owl:DatatypeProperty rdf:about="http://example.org/onto/prop/google_container_cluster_transparent_hugepage_enabled">
    <rdfs:label>transparent_hugepage_enabled</rdfs:label>
    <rdfs:comment>The Linux kernel transparent hugepage setting.</rdfs:comment>
    <rdfs:domain rdf:resource="http://example.org/onto/class/google_container_cluster"/>
    <rdfs:range rdf:resource="http://www.w3.org/2001/XMLSchema#string"/>
  </owl:DatatypeProperty>
  <owl:DatatypeProperty rdf:about="http://example.org/onto/prop/google_container_cluster_hugepage_size_1g">
    <rdfs:label>hugepage_size_1g</rdfs:label>
    <rdfs:comment>Amount of 1G hugepages.</rdfs:comment>
    <rdfs:domain rdf:resource="http://example.org/onto/class/google_container_cluster"/>
    <rdfs:range rdf:resource="http://www.w3.org/2001/XMLSchema#string"/>
  </owl:DatatypeProperty>
  <owl:DatatypeProperty rdf:about="http://example.org/onto/prop/google_container_cluster_hugepage_size_2m">
    <rdfs:label>hugepage_size_2m</rdfs:label>
    <rdfs:comment>Amount of 2M hugepages.</rdfs:comment>
    <rdfs:domain rdf:resource="http://example.org/onto/class/google_container_cluster"/>
    <rdfs:range rdf:resource="http://www.w3.org/2001/XMLSchema#string"/>
  </owl:DatatypeProperty>
  <owl:DatatypeProperty rdf:about="http://example.org/onto/prop/google_container_cluster_local_ssd_count">
    <rdfs:label>local_ssd_count</rdfs:label>
    <rdfs:comment>Number of raw-block local NVMe SSD disks to be attached to the node. Each local SSD is 375 GB in size.</rdfs:comment>
    <rdfs:domain rdf:resource="http://example.org/onto/class/google_container_cluster"/>
    <rdfs:range rdf:resource="http://www.w3.org/2001/XMLSchema#string"/>
  </owl:DatatypeProperty>
  <owl:DatatypeProperty rdf:about="http://example.org/onto/prop/google_container_cluster_consume_reservation_type">
    <rdfs:label>consume_reservation_type</rdfs:label>
    <rdfs:comment>Corresponds to the type of reservation consumption.</rdfs:comment>
    <rdfs:domain rdf:resource="http://example.org/onto/class/google_container_cluster"/>
    <rdfs:range rdf:resource="http://www.w3.org/2001/XMLSchema#string"/>
  </owl:DatatypeProperty>
  <owl:DatatypeProperty rdf:about="http://example.org/onto/prop/google_container_cluster_key">
    <rdfs:label>key</rdfs:label>
    <rdfs:comment>The label key of a reservation resource.</rdfs:comment>
    <rdfs:domain rdf:resource="http://example.org/onto/class/google_container_cluster"/>
    <rdfs:range rdf:resource="http://www.w3.org/2001/XMLSchema#string"/>
  </owl:DatatypeProperty>
  <owl:DatatypeProperty rdf:about="http://example.org/onto/prop/google_container_cluster_values">
    <rdfs:label>values</rdfs:label>
    <rdfs:comment>The label values of the reservation resource.</rdfs:comment>
    <rdfs:domain rdf:resource="http://example.org/onto/class/google_container_cluster"/>
    <rdfs:range rdf:resource="http://www.w3.org/2001/XMLSchema#string"/>
  </owl:DatatypeProperty>
  <owl:DatatypeProperty rdf:about="http://example.org/onto/prop/google_container_cluster_disk_image">
    <rdfs:label>disk_image</rdfs:label>
    <rdfs:comment>Disk image to create the secondary boot disk from</rdfs:comment>
    <rdfs:domain rdf:resource="http://example.org/onto/class/google_container_cluster"/>
    <rdfs:range rdf:resource="http://www.w3.org/2001/XMLSchema#string"/>
  </owl:DatatypeProperty>
  <owl:DatatypeProperty rdf:about="http://example.org/onto/prop/google_container_cluster_mode">
    <rdfs:label>mode</rdfs:label>
    <rdfs:comment>Mode for how the secondary boot disk is used.</rdfs:comment>
    <rdfs:domain rdf:resource="http://example.org/onto/class/google_container_cluster"/>
    <rdfs:range rdf:resource="http://www.w3.org/2001/XMLSchema#string"/>
  </owl:DatatypeProperty>
  <owl:DatatypeProperty rdf:about="http://example.org/onto/prop/google_container_cluster_enable_integrity_monitoring">
    <rdfs:label>enable_integrity_monitoring</rdfs:label>
    <rdfs:comment>Defines whether the instance has integrity monitoring enabled.</rdfs:comment>
    <rdfs:domain rdf:resource="http://example.org/onto/class/google_container_cluster"/>
    <rdfs:range rdf:resource="http://www.w3.org/2001/XMLSchema#string"/>
  </owl:DatatypeProperty>
  <owl:DatatypeProperty rdf:about="http://example.org/onto/prop/google_container_cluster_enable_secure_boot">
    <rdfs:label>enable_secure_boot</rdfs:label>
    <rdfs:comment>Defines whether the instance has Secure Boot enabled.</rdfs:comment>
    <rdfs:domain rdf:resource="http://example.org/onto/class/google_container_cluster"/>
    <rdfs:range rdf:resource="http://www.w3.org/2001/XMLSchema#string"/>
  </owl:DatatypeProperty>
  <owl:DatatypeProperty rdf:about="http://example.org/onto/prop/google_container_cluster_min_node_cpus">
    <rdfs:label>min_node_cpus</rdfs:label>
    <rdfs:comment>Specifies the minimum number of vCPUs that each sole tenant node must have to use CPU overcommit. If not specified, the CPU overcommit feature is disabled.</rdfs:comment>
    <rdfs:domain rdf:resource="http://example.org/onto/class/google_container_cluster"/>
    <rdfs:range rdf:resource="http://www.w3.org/2001/XMLSchema#string"/>
  </owl:DatatypeProperty>
  <owl:DatatypeProperty rdf:about="http://example.org/onto/prop/google_container_cluster_key">
    <rdfs:label>key</rdfs:label>
    <rdfs:comment>.</rdfs:comment>
    <rdfs:domain rdf:resource="http://example.org/onto/class/google_container_cluster"/>
    <rdfs:range rdf:resource="http://www.w3.org/2001/XMLSchema#string"/>
  </owl:DatatypeProperty>
  <owl:DatatypeProperty rdf:about="http://example.org/onto/prop/google_container_cluster_operator">
    <rdfs:label>operator</rdfs:label>
    <rdfs:comment>.</rdfs:comment>
    <rdfs:domain rdf:resource="http://example.org/onto/class/google_container_cluster"/>
    <rdfs:range rdf:resource="http://www.w3.org/2001/XMLSchema#string"/>
  </owl:DatatypeProperty>
  <owl:DatatypeProperty rdf:about="http://example.org/onto/prop/google_container_cluster_values">
    <rdfs:label>values</rdfs:label>
    <rdfs:comment>.</rdfs:comment>
    <rdfs:domain rdf:resource="http://example.org/onto/class/google_container_cluster"/>
    <rdfs:range rdf:resource="http://www.w3.org/2001/XMLSchema#string"/>
  </owl:DatatypeProperty>
  <owl:DatatypeProperty rdf:about="http://example.org/onto/prop/google_container_cluster_effect">
    <rdfs:label>effect</rdfs:label>
    <rdfs:comment>Effect for taint.</rdfs:comment>
    <rdfs:domain rdf:resource="http://example.org/onto/class/google_container_cluster"/>
    <rdfs:range rdf:resource="http://www.w3.org/2001/XMLSchema#string"/>
  </owl:DatatypeProperty>
  <owl:DatatypeProperty rdf:about="http://example.org/onto/prop/google_container_cluster_key">
    <rdfs:label>key</rdfs:label>
    <rdfs:comment>Key for taint.</rdfs:comment>
    <rdfs:domain rdf:resource="http://example.org/onto/class/google_container_cluster"/>
    <rdfs:range rdf:resource="http://www.w3.org/2001/XMLSchema#string"/>
  </owl:DatatypeProperty>
  <owl:DatatypeProperty rdf:about="http://example.org/onto/prop/google_container_cluster_value">
    <rdfs:label>value</rdfs:label>
    <rdfs:comment>Value for taint.</rdfs:comment>
    <rdfs:domain rdf:resource="http://example.org/onto/class/google_container_cluster"/>
    <rdfs:range rdf:resource="http://www.w3.org/2001/XMLSchema#string"/>
  </owl:DatatypeProperty>
  <owl:DatatypeProperty rdf:about="http://example.org/onto/prop/google_container_cluster_osversion">
    <rdfs:label>osversion</rdfs:label>
    <rdfs:comment>The OS Version of the windows nodepool.Values are OS_VERSION_UNSPECIFIED,OS_VERSION_LTSC2019 and OS_VERSION_LTSC2022</rdfs:comment>
    <rdfs:domain rdf:resource="http://example.org/onto/class/google_container_cluster"/>
    <rdfs:range rdf:resource="http://www.w3.org/2001/XMLSchema#string"/>
  </owl:DatatypeProperty>
  <owl:DatatypeProperty rdf:about="http://example.org/onto/prop/google_container_cluster_mode">
    <rdfs:label>mode</rdfs:label>
    <rdfs:comment>Mode is the configuration for how to expose metadata to workloads running on the node.</rdfs:comment>
    <rdfs:domain rdf:resource="http://example.org/onto/class/google_container_cluster"/>
    <rdfs:range rdf:resource="http://www.w3.org/2001/XMLSchema#string"/>
  </owl:DatatypeProperty>
  <owl:DatatypeProperty rdf:about="http://example.org/onto/prop/google_container_cluster_initial_node_count">
    <rdfs:label>initial_node_count</rdfs:label>
    <rdfs:comment>The initial number of nodes for the pool. In regional or multi-zonal clusters, this is the number of nodes per zone. Changing this will force recreation of the resource.</rdfs:comment>
    <rdfs:domain rdf:resource="http://example.org/onto/class/google_container_cluster"/>
    <rdfs:range rdf:resource="http://www.w3.org/2001/XMLSchema#string"/>
  </owl:DatatypeProperty>
  <owl:DatatypeProperty rdf:about="http://example.org/onto/prop/google_container_cluster_instance_group_urls">
    <rdfs:label>instance_group_urls</rdfs:label>
    <rdfs:comment>The resource URLs of the managed instance groups associated with this node pool.</rdfs:comment>
    <rdfs:domain rdf:resource="http://example.org/onto/class/google_container_cluster"/>
    <rdfs:range rdf:resource="http://www.w3.org/2001/XMLSchema#string"/>
  </owl:DatatypeProperty>
  <owl:DatatypeProperty rdf:about="http://example.org/onto/prop/google_container_cluster_managed_instance_group_urls">
    <rdfs:label>managed_instance_group_urls</rdfs:label>
    <rdfs:comment>List of instance group URLs which have been assigned to this node pool.</rdfs:comment>
    <rdfs:domain rdf:resource="http://example.org/onto/class/google_container_cluster"/>
    <rdfs:range rdf:resource="http://www.w3.org/2001/XMLSchema#string"/>
  </owl:DatatypeProperty>
  <owl:DatatypeProperty rdf:about="http://example.org/onto/prop/google_container_cluster_max_pods_per_node">
    <rdfs:label>max_pods_per_node</rdfs:label>
    <rdfs:comment>The maximum number of pods per node in this node pool. Note that this does not work on node pools which are "route-based" - that is, node pools belonging to clusters that do not have IP Aliasing enabled.</rdfs:comment>
    <rdfs:domain rdf:resource="http://example.org/onto/class/google_container_cluster"/>
    <rdfs:range rdf:resource="http://www.w3.org/2001/XMLSchema#string"/>
  </owl:DatatypeProperty>
  <owl:DatatypeProperty rdf:about="http://example.org/onto/prop/google_container_cluster_name">
    <rdfs:label>name</rdfs:label>
    <rdfs:comment>The name of the node pool. If left blank, Terraform will auto-generate a unique name.</rdfs:comment>
    <rdfs:domain rdf:resource="http://example.org/onto/class/google_container_cluster"/>
    <rdfs:range rdf:resource="http://www.w3.org/2001/XMLSchema#string"/>
  </owl:DatatypeProperty>
  <owl:DatatypeProperty rdf:about="http://example.org/onto/prop/google_container_cluster_name_prefix">
    <rdfs:label>name_prefix</rdfs:label>
    <rdfs:comment>Creates a unique name for the node pool beginning with the specified prefix. Conflicts with name.</rdfs:comment>
    <rdfs:domain rdf:resource="http://example.org/onto/class/google_container_cluster"/>
    <rdfs:range rdf:resource="http://www.w3.org/2001/XMLSchema#string"/>
  </owl:DatatypeProperty>
  <owl:DatatypeProperty rdf:about="http://example.org/onto/prop/google_container_cluster_node_count">
    <rdfs:label>node_count</rdfs:label>
    <rdfs:comment>The number of nodes per instance group. This field can be used to update the number of nodes per instance group but should not be used alongside autoscaling.</rdfs:comment>
    <rdfs:domain rdf:resource="http://example.org/onto/class/google_container_cluster"/>
    <rdfs:range rdf:resource="http://www.w3.org/2001/XMLSchema#string"/>
  </owl:DatatypeProperty>
  <owl:DatatypeProperty rdf:about="http://example.org/onto/prop/google_container_cluster_node_locations">
    <rdfs:label>node_locations</rdfs:label>
    <rdfs:comment>The list of zones in which the node pool's nodes should be located. Nodes must be in the region of their regional cluster or in the same region as their cluster's zone for zonal clusters. If unspecified, the cluster-level node_locations will be used.</rdfs:comment>
    <rdfs:domain rdf:resource="http://example.org/onto/class/google_container_cluster"/>
    <rdfs:range rdf:resource="http://www.w3.org/2001/XMLSchema#string"/>
  </owl:DatatypeProperty>
  <owl:DatatypeProperty rdf:about="http://example.org/onto/prop/google_container_cluster_version">
    <rdfs:label>version</rdfs:label>
    <rdfs:comment>The Kubernetes version for the nodes in this pool. Note that if this field and auto_upgrade are both specified, they will fight each other for what the node version should be, so setting both is highly discouraged. While a fuzzy version can be specified, it's recommended that you specify explicit versions as Terraform will see spurious diffs when fuzzy versions are used. See the google_container_engine_versions data source's version_prefix field to approximate fuzzy versions in a Terraform-compatible way.</rdfs:comment>
    <rdfs:domain rdf:resource="http://example.org/onto/class/google_container_cluster"/>
    <rdfs:range rdf:resource="http://www.w3.org/2001/XMLSchema#string"/>
  </owl:DatatypeProperty>
  <owl:DatatypeProperty rdf:about="http://example.org/onto/prop/google_container_cluster_location_policy">
    <rdfs:label>location_policy</rdfs:label>
    <rdfs:comment>Location policy specifies the algorithm used when scaling-up the node pool. "BALANCED" - Is a best effort policy that aims to balance the sizes of available zones. "ANY" - Instructs the cluster autoscaler to prioritize utilization of unused reservations, and reduces preemption risk for Spot VMs.</rdfs:comment>
    <rdfs:domain rdf:resource="http://example.org/onto/class/google_container_cluster"/>
    <rdfs:range rdf:resource="http://www.w3.org/2001/XMLSchema#string"/>
  </owl:DatatypeProperty>
  <owl:DatatypeProperty rdf:about="http://example.org/onto/prop/google_container_cluster_max_node_count">
    <rdfs:label>max_node_count</rdfs:label>
    <rdfs:comment>Maximum number of nodes per zone in the node pool. Must be >= min_node_count. Cannot be used with total limits.</rdfs:comment>
    <rdfs:domain rdf:resource="http://example.org/onto/class/google_container_cluster"/>
    <rdfs:range rdf:resource="http://www.w3.org/2001/XMLSchema#string"/>
  </owl:DatatypeProperty>
  <owl:DatatypeProperty rdf:about="http://example.org/onto/prop/google_container_cluster_min_node_count">
    <rdfs:label>min_node_count</rdfs:label>
    <rdfs:comment>Minimum number of nodes per zone in the node pool. Must be >=0 and <= max_node_count. Cannot be used with total limits.</rdfs:comment>
    <rdfs:domain rdf:resource="http://example.org/onto/class/google_container_cluster"/>
    <rdfs:range rdf:resource="http://www.w3.org/2001/XMLSchema#string"/>
  </owl:DatatypeProperty>
  <owl:DatatypeProperty rdf:about="http://example.org/onto/prop/google_container_cluster_total_max_node_count">
    <rdfs:label>total_max_node_count</rdfs:label>
    <rdfs:comment>Maximum number of all nodes in the node pool. Must be >= total_min_node_count. Cannot be used with per zone limits.</rdfs:comment>
    <rdfs:domain rdf:resource="http://example.org/onto/class/google_container_cluster"/>
    <rdfs:range rdf:resource="http://www.w3.org/2001/XMLSchema#string"/>
  </owl:DatatypeProperty>
  <owl:DatatypeProperty rdf:about="http://example.org/onto/prop/google_container_cluster_total_min_node_count">
    <rdfs:label>total_min_node_count</rdfs:label>
    <rdfs:comment>Minimum number of all nodes in the node pool. Must be >=0 and <= total_max_node_count. Cannot be used with per zone limits.</rdfs:comment>
    <rdfs:domain rdf:resource="http://example.org/onto/class/google_container_cluster"/>
    <rdfs:range rdf:resource="http://www.w3.org/2001/XMLSchema#string"/>
  </owl:DatatypeProperty>
  <owl:DatatypeProperty rdf:about="http://example.org/onto/prop/google_container_cluster_auto_repair">
    <rdfs:label>auto_repair</rdfs:label>
    <rdfs:comment>Whether the nodes will be automatically repaired. Enabled by default.</rdfs:comment>
    <rdfs:domain rdf:resource="http://example.org/onto/class/google_container_cluster"/>
    <rdfs:range rdf:resource="http://www.w3.org/2001/XMLSchema#string"/>
  </owl:DatatypeProperty>
  <owl:DatatypeProperty rdf:about="http://example.org/onto/prop/google_container_cluster_auto_upgrade">
    <rdfs:label>auto_upgrade</rdfs:label>
    <rdfs:comment>Whether the nodes will be automatically upgraded. Enabled by default.</rdfs:comment>
    <rdfs:domain rdf:resource="http://example.org/onto/class/google_container_cluster"/>
    <rdfs:range rdf:resource="http://www.w3.org/2001/XMLSchema#string"/>
  </owl:DatatypeProperty>
  <owl:DatatypeProperty rdf:about="http://example.org/onto/prop/google_container_cluster_create_pod_range">
    <rdfs:label>create_pod_range</rdfs:label>
    <rdfs:comment>Whether to create a new range for pod IPs in this node pool. Defaults are provided for pod_range and pod_ipv4_cidr_block if they are not specified.</rdfs:comment>
    <rdfs:domain rdf:resource="http://example.org/onto/class/google_container_cluster"/>
    <rdfs:range rdf:resource="http://www.w3.org/2001/XMLSchema#string"/>
  </owl:DatatypeProperty>
  <owl:DatatypeProperty rdf:about="http://example.org/onto/prop/google_container_cluster_enable_private_nodes">
    <rdfs:label>enable_private_nodes</rdfs:label>
    <rdfs:comment>Whether nodes have internal IP addresses only.</rdfs:comment>
    <rdfs:domain rdf:resource="http://example.org/onto/class/google_container_cluster"/>
    <rdfs:range rdf:resource="http://www.w3.org/2001/XMLSchema#string"/>
  </owl:DatatypeProperty>
  <owl:DatatypeProperty rdf:about="http://example.org/onto/prop/google_container_cluster_pod_ipv4_cidr_block">
    <rdfs:label>pod_ipv4_cidr_block</rdfs:label>
    <rdfs:comment>The IP address range for pod IPs in this node pool. Only applicable if create_pod_range is true. Set to blank to have a range chosen with the default size. Set to /netmask (e.g. /14) to have a range chosen with a specific netmask. Set to a CIDR notation (e.g. 10.96.0.0/14) to pick a specific range to use.</rdfs:comment>
    <rdfs:domain rdf:resource="http://example.org/onto/class/google_container_cluster"/>
    <rdfs:range rdf:resource="http://www.w3.org/2001/XMLSchema#string"/>
  </owl:DatatypeProperty>
  <owl:DatatypeProperty rdf:about="http://example.org/onto/prop/google_container_cluster_pod_range">
    <rdfs:label>pod_range</rdfs:label>
    <rdfs:comment>The ID of the secondary range for pod IPs. If create_pod_range is true, this ID is used for the new range. If create_pod_range is false, uses an existing secondary range with this ID.</rdfs:comment>
    <rdfs:domain rdf:resource="http://example.org/onto/class/google_container_cluster"/>
    <rdfs:range rdf:resource="http://www.w3.org/2001/XMLSchema#string"/>
  </owl:DatatypeProperty>
  <owl:DatatypeProperty rdf:about="http://example.org/onto/prop/google_container_cluster_subnetwork">
    <rdfs:label>subnetwork</rdfs:label>
    <rdfs:comment>The subnetwork path for the node pool. Format: projects/{project}/regions/{region}/subnetworks/{subnetwork} . If the cluster is associated with multiple subnetworks, the subnetwork for the node pool is picked based on the IP utilization during node pool creation and is immutable.</rdfs:comment>
    <rdfs:domain rdf:resource="http://example.org/onto/class/google_container_cluster"/>
    <rdfs:range rdf:resource="http://www.w3.org/2001/XMLSchema#string"/>
  </owl:DatatypeProperty>
  <owl:DatatypeProperty rdf:about="http://example.org/onto/prop/google_container_cluster_network">
    <rdfs:label>network</rdfs:label>
    <rdfs:comment>Name of the VPC where the additional interface belongs.</rdfs:comment>
    <rdfs:domain rdf:resource="http://example.org/onto/class/google_container_cluster"/>
    <rdfs:range rdf:resource="http://www.w3.org/2001/XMLSchema#string"/>
  </owl:DatatypeProperty>
  <owl:DatatypeProperty rdf:about="http://example.org/onto/prop/google_container_cluster_subnetwork">
    <rdfs:label>subnetwork</rdfs:label>
    <rdfs:comment>Name of the subnetwork where the additional interface belongs.</rdfs:comment>
    <rdfs:domain rdf:resource="http://example.org/onto/class/google_container_cluster"/>
    <rdfs:range rdf:resource="http://www.w3.org/2001/XMLSchema#string"/>
  </owl:DatatypeProperty>
  <owl:DatatypeProperty rdf:about="http://example.org/onto/prop/google_container_cluster_max_pods_per_node">
    <rdfs:label>max_pods_per_node</rdfs:label>
    <rdfs:comment>The maximum number of pods per node which use this pod network.</rdfs:comment>
    <rdfs:domain rdf:resource="http://example.org/onto/class/google_container_cluster"/>
    <rdfs:range rdf:resource="http://www.w3.org/2001/XMLSchema#string"/>
  </owl:DatatypeProperty>
  <owl:DatatypeProperty rdf:about="http://example.org/onto/prop/google_container_cluster_secondary_pod_range">
    <rdfs:label>secondary_pod_range</rdfs:label>
    <rdfs:comment>The name of the secondary range on the subnet which provides IP address for this pod range.</rdfs:comment>
    <rdfs:domain rdf:resource="http://example.org/onto/class/google_container_cluster"/>
    <rdfs:range rdf:resource="http://www.w3.org/2001/XMLSchema#string"/>
  </owl:DatatypeProperty>
  <owl:DatatypeProperty rdf:about="http://example.org/onto/prop/google_container_cluster_subnetwork">
    <rdfs:label>subnetwork</rdfs:label>
    <rdfs:comment>Name of the subnetwork where the additional pod network belongs.</rdfs:comment>
    <rdfs:domain rdf:resource="http://example.org/onto/class/google_container_cluster"/>
    <rdfs:range rdf:resource="http://www.w3.org/2001/XMLSchema#string"/>
  </owl:DatatypeProperty>
  <owl:DatatypeProperty rdf:about="http://example.org/onto/prop/google_container_cluster_total_egress_bandwidth_tier">
    <rdfs:label>total_egress_bandwidth_tier</rdfs:label>
    <rdfs:comment>Specifies the total network bandwidth tier for the NodePool. [Valid values](https://cloud.google.com/kubernetes-engine/docs/reference/rest/v1/projects.locations.clusters.nodePools#NodePool.Tier) include: "TIER_1" and "TIER_UNSPECIFIED".</rdfs:comment>
    <rdfs:domain rdf:resource="http://example.org/onto/class/google_container_cluster"/>
    <rdfs:range rdf:resource="http://www.w3.org/2001/XMLSchema#string"/>
  </owl:DatatypeProperty>
  <owl:DatatypeProperty rdf:about="http://example.org/onto/prop/google_container_cluster_disabled">
    <rdfs:label>disabled</rdfs:label>
    <rdfs:domain rdf:resource="http://example.org/onto/class/google_container_cluster"/>
    <rdfs:range rdf:resource="http://www.w3.org/2001/XMLSchema#string"/>
  </owl:DatatypeProperty>
  <owl:DatatypeProperty rdf:about="http://example.org/onto/prop/google_container_cluster_boot_disk_kms_key">
    <rdfs:label>boot_disk_kms_key</rdfs:label>
    <rdfs:comment>The Customer Managed Encryption Key used to encrypt the boot disk attached to each node in the node pool.</rdfs:comment>
    <rdfs:domain rdf:resource="http://example.org/onto/class/google_container_cluster"/>
    <rdfs:range rdf:resource="http://www.w3.org/2001/XMLSchema#string"/>
  </owl:DatatypeProperty>
  <owl:DatatypeProperty rdf:about="http://example.org/onto/prop/google_container_cluster_disk_size_gb">
    <rdfs:label>disk_size_gb</rdfs:label>
    <rdfs:comment>Size of the disk attached to each node, specified in GB. The smallest allowed disk size is 10GB.</rdfs:comment>
    <rdfs:domain rdf:resource="http://example.org/onto/class/google_container_cluster"/>
    <rdfs:range rdf:resource="http://www.w3.org/2001/XMLSchema#string"/>
  </owl:DatatypeProperty>
  <owl:DatatypeProperty rdf:about="http://example.org/onto/prop/google_container_cluster_disk_type">
    <rdfs:label>disk_type</rdfs:label>
    <rdfs:comment>Type of the disk attached to each node. Such as pd-standard, pd-balanced or pd-ssd</rdfs:comment>
    <rdfs:domain rdf:resource="http://example.org/onto/class/google_container_cluster"/>
    <rdfs:range rdf:resource="http://www.w3.org/2001/XMLSchema#string"/>
  </owl:DatatypeProperty>
  <owl:DatatypeProperty rdf:about="http://example.org/onto/prop/google_container_cluster_effective_taints">
    <rdfs:label>effective_taints</rdfs:label>
    <rdfs:comment>List of kubernetes taints applied to each node.</rdfs:comment>
    <rdfs:domain rdf:resource="http://example.org/onto/class/google_container_cluster"/>
    <rdfs:range rdf:resource="http://www.w3.org/2001/XMLSchema#string"/>
  </owl:DatatypeProperty>
  <owl:DatatypeProperty rdf:about="http://example.org/onto/prop/google_container_cluster_enable_confidential_storage">
    <rdfs:label>enable_confidential_storage</rdfs:label>
    <rdfs:comment>If enabled boot disks are configured with confidential mode.</rdfs:comment>
    <rdfs:domain rdf:resource="http://example.org/onto/class/google_container_cluster"/>
    <rdfs:range rdf:resource="http://www.w3.org/2001/XMLSchema#string"/>
  </owl:DatatypeProperty>
  <owl:DatatypeProperty rdf:about="http://example.org/onto/prop/google_container_cluster_flex_start">
    <rdfs:label>flex_start</rdfs:label>
    <rdfs:comment>Enables Flex Start provisioning model for the node pool</rdfs:comment>
    <rdfs:domain rdf:resource="http://example.org/onto/class/google_container_cluster"/>
    <rdfs:range rdf:resource="http://www.w3.org/2001/XMLSchema#string"/>
  </owl:DatatypeProperty>
  <owl:DatatypeProperty rdf:about="http://example.org/onto/prop/google_container_cluster_image_type">
    <rdfs:label>image_type</rdfs:label>
    <rdfs:comment>The image type to use for this node. Note that for a given image type, the latest version of it will be used.</rdfs:comment>
    <rdfs:domain rdf:resource="http://example.org/onto/class/google_container_cluster"/>
    <rdfs:range rdf:resource="http://www.w3.org/2001/XMLSchema#string"/>
  </owl:DatatypeProperty>
  <owl:DatatypeProperty rdf:about="http://example.org/onto/prop/google_container_cluster_labels">
    <rdfs:label>labels</rdfs:label>
    <rdfs:comment>The map of Kubernetes labels (key/value pairs) to be applied to each node. These will added in addition to any default label(s) that Kubernetes may apply to the node.</rdfs:comment>
    <rdfs:domain rdf:resource="http://example.org/onto/class/google_container_cluster"/>
    <rdfs:range rdf:resource="http://www.w3.org/2001/XMLSchema#string"/>
  </owl:DatatypeProperty>
  <owl:DatatypeProperty rdf:about="http://example.org/onto/prop/google_container_cluster_local_ssd_count">
    <rdfs:label>local_ssd_count</rdfs:label>
    <rdfs:comment>The number of local SSD disks to be attached to the node.</rdfs:comment>
    <rdfs:domain rdf:resource="http://example.org/onto/class/google_container_cluster"/>
    <rdfs:range rdf:resource="http://www.w3.org/2001/XMLSchema#string"/>
  </owl:DatatypeProperty>
  <owl:DatatypeProperty rdf:about="http://example.org/onto/prop/google_container_cluster_local_ssd_encryption_mode">
    <rdfs:label>local_ssd_encryption_mode</rdfs:label>
    <rdfs:comment>LocalSsdEncryptionMode specified the method used for encrypting the local SSDs attached to the node.</rdfs:comment>
    <rdfs:domain rdf:resource="http://example.org/onto/class/google_container_cluster"/>
    <rdfs:range rdf:resource="http://www.w3.org/2001/XMLSchema#string"/>
  </owl:DatatypeProperty>
  <owl:DatatypeProperty rdf:about="http://example.org/onto/prop/google_container_cluster_logging_variant">
    <rdfs:label>logging_variant</rdfs:label>
    <rdfs:comment>Type of logging agent that is used as the default value for node pools in the cluster. Valid values include DEFAULT and MAX_THROUGHPUT.</rdfs:comment>
    <rdfs:domain rdf:resource="http://example.org/onto/class/google_container_cluster"/>
    <rdfs:range rdf:resource="http://www.w3.org/2001/XMLSchema#string"/>
  </owl:DatatypeProperty>
  <owl:DatatypeProperty rdf:about="http://example.org/onto/prop/google_container_cluster_machine_type">
    <rdfs:label>machine_type</rdfs:label>
    <rdfs:comment>The name of a Google Compute Engine machine type.</rdfs:comment>
    <rdfs:domain rdf:resource="http://example.org/onto/class/google_container_cluster"/>
    <rdfs:range rdf:resource="http://www.w3.org/2001/XMLSchema#string"/>
  </owl:DatatypeProperty>
  <owl:DatatypeProperty rdf:about="http://example.org/onto/prop/google_container_cluster_max_run_duration">
    <rdfs:label>max_run_duration</rdfs:label>
    <rdfs:comment>The runtime of each node in the node pool in seconds, terminated by 's'. Example: "3600s".</rdfs:comment>
    <rdfs:domain rdf:resource="http://example.org/onto/class/google_container_cluster"/>
    <rdfs:range rdf:resource="http://www.w3.org/2001/XMLSchema#string"/>
  </owl:DatatypeProperty>
  <owl:DatatypeProperty rdf:about="http://example.org/onto/prop/google_container_cluster_metadata">
    <rdfs:label>metadata</rdfs:label>
    <rdfs:comment>The metadata key/value pairs assigned to instances in the cluster.</rdfs:comment>
    <rdfs:domain rdf:resource="http://example.org/onto/class/google_container_cluster"/>
    <rdfs:range rdf:resource="http://www.w3.org/2001/XMLSchema#string"/>
  </owl:DatatypeProperty>
  <owl:DatatypeProperty rdf:about="http://example.org/onto/prop/google_container_cluster_min_cpu_platform">
    <rdfs:label>min_cpu_platform</rdfs:label>
    <rdfs:comment>Minimum CPU platform to be used by this instance. The instance may be scheduled on the specified or newer CPU platform.</rdfs:comment>
    <rdfs:domain rdf:resource="http://example.org/onto/class/google_container_cluster"/>
    <rdfs:range rdf:resource="http://www.w3.org/2001/XMLSchema#string"/>
  </owl:DatatypeProperty>
  <owl:DatatypeProperty rdf:about="http://example.org/onto/prop/google_container_cluster_node_group">
    <rdfs:label>node_group</rdfs:label>
    <rdfs:comment>Setting this field will assign instances of this pool to run on the specified node group. This is useful for running workloads on sole tenant nodes.</rdfs:comment>
    <rdfs:domain rdf:resource="http://example.org/onto/class/google_container_cluster"/>
    <rdfs:range rdf:resource="http://www.w3.org/2001/XMLSchema#string"/>
  </owl:DatatypeProperty>
  <owl:DatatypeProperty rdf:about="http://example.org/onto/prop/google_container_cluster_oauth_scopes">
    <rdfs:label>oauth_scopes</rdfs:label>
    <rdfs:comment>The set of Google API scopes to be made available on all of the node VMs.</rdfs:comment>
    <rdfs:domain rdf:resource="http://example.org/onto/class/google_container_cluster"/>
    <rdfs:range rdf:resource="http://www.w3.org/2001/XMLSchema#string"/>
  </owl:DatatypeProperty>
  <owl:DatatypeProperty rdf:about="http://example.org/onto/prop/google_container_cluster_preemptible">
    <rdfs:label>preemptible</rdfs:label>
    <rdfs:comment>Whether the nodes are created as preemptible VM instances.</rdfs:comment>
    <rdfs:domain rdf:resource="http://example.org/onto/class/google_container_cluster"/>
    <rdfs:range rdf:resource="http://www.w3.org/2001/XMLSchema#string"/>
  </owl:DatatypeProperty>
  <owl:DatatypeProperty rdf:about="http://example.org/onto/prop/google_container_cluster_resource_labels">
    <rdfs:label>resource_labels</rdfs:label>
    <rdfs:comment>The GCE resource labels (a map of key/value pairs) to be applied to the node pool.</rdfs:comment>
    <rdfs:domain rdf:resource="http://example.org/onto/class/google_container_cluster"/>
    <rdfs:range rdf:resource="http://www.w3.org/2001/XMLSchema#string"/>
  </owl:DatatypeProperty>
  <owl:DatatypeProperty rdf:about="http://example.org/onto/prop/google_container_cluster_resource_manager_tags">
    <rdfs:label>resource_manager_tags</rdfs:label>
    <rdfs:comment>A map of resource manager tags. Resource manager tag keys and values have the same definition as resource manager tags. Keys must be in the format tagKeys/{tag_key_id}, and values are in the format tagValues/456. The field is ignored (both PUT & PATCH) when empty.</rdfs:comment>
    <rdfs:domain rdf:resource="http://example.org/onto/class/google_container_cluster"/>
    <rdfs:range rdf:resource="http://www.w3.org/2001/XMLSchema#string"/>
  </owl:DatatypeProperty>
  <owl:DatatypeProperty rdf:about="http://example.org/onto/prop/google_container_cluster_service_account">
    <rdfs:label>service_account</rdfs:label>
    <rdfs:comment>The Google Cloud Platform Service Account to be used by the node VMs.</rdfs:comment>
    <rdfs:domain rdf:resource="http://example.org/onto/class/google_container_cluster"/>
    <rdfs:range rdf:resource="http://www.w3.org/2001/XMLSchema#string"/>
  </owl:DatatypeProperty>
  <owl:DatatypeProperty rdf:about="http://example.org/onto/prop/google_container_cluster_spot">
    <rdfs:label>spot</rdfs:label>
    <rdfs:comment>Whether the nodes are created as spot VM instances.</rdfs:comment>
    <rdfs:domain rdf:resource="http://example.org/onto/class/google_container_cluster"/>
    <rdfs:range rdf:resource="http://www.w3.org/2001/XMLSchema#string"/>
  </owl:DatatypeProperty>
  <owl:DatatypeProperty rdf:about="http://example.org/onto/prop/google_container_cluster_storage_pools">
    <rdfs:label>storage_pools</rdfs:label>
    <rdfs:comment>The list of Storage Pools where boot disks are provisioned.</rdfs:comment>
    <rdfs:domain rdf:resource="http://example.org/onto/class/google_container_cluster"/>
    <rdfs:range rdf:resource="http://www.w3.org/2001/XMLSchema#string"/>
  </owl:DatatypeProperty>
  <owl:DatatypeProperty rdf:about="http://example.org/onto/prop/google_container_cluster_tags">
    <rdfs:label>tags</rdfs:label>
    <rdfs:comment>The list of instance tags applied to all nodes.</rdfs:comment>
    <rdfs:domain rdf:resource="http://example.org/onto/class/google_container_cluster"/>
    <rdfs:range rdf:resource="http://www.w3.org/2001/XMLSchema#string"/>
  </owl:DatatypeProperty>
  <owl:DatatypeProperty rdf:about="http://example.org/onto/prop/google_container_cluster_enable_nested_virtualization">
    <rdfs:label>enable_nested_virtualization</rdfs:label>
    <rdfs:comment>Whether the node should have nested virtualization enabled.</rdfs:comment>
    <rdfs:domain rdf:resource="http://example.org/onto/class/google_container_cluster"/>
    <rdfs:range rdf:resource="http://www.w3.org/2001/XMLSchema#string"/>
  </owl:DatatypeProperty>
  <owl:DatatypeProperty rdf:about="http://example.org/onto/prop/google_container_cluster_performance_monitoring_unit">
    <rdfs:label>performance_monitoring_unit</rdfs:label>
    <rdfs:comment>Level of Performance Monitoring Unit (PMU) requested. If unset, no access to the PMU is assumed.</rdfs:comment>
    <rdfs:domain rdf:resource="http://example.org/onto/class/google_container_cluster"/>
    <rdfs:range rdf:resource="http://www.w3.org/2001/XMLSchema#string"/>
  </owl:DatatypeProperty>
  <owl:DatatypeProperty rdf:about="http://example.org/onto/prop/google_container_cluster_threads_per_core">
    <rdfs:label>threads_per_core</rdfs:label>
    <rdfs:comment>The number of threads per physical core. To disable simultaneous multithreading (SMT) set this to 1. If unset, the maximum number of threads supported per core by the underlying processor is assumed.</rdfs:comment>
    <rdfs:domain rdf:resource="http://example.org/onto/class/google_container_cluster"/>
    <rdfs:range rdf:resource="http://www.w3.org/2001/XMLSchema#string"/>
  </owl:DatatypeProperty>
  <owl:DatatypeProperty rdf:about="http://example.org/onto/prop/google_container_cluster_disk_type">
    <rdfs:label>disk_type</rdfs:label>
    <rdfs:comment>Type of the disk attached to each node. Such as pd-standard, pd-balanced or pd-ssd</rdfs:comment>
    <rdfs:domain rdf:resource="http://example.org/onto/class/google_container_cluster"/>
    <rdfs:range rdf:resource="http://www.w3.org/2001/XMLSchema#string"/>
  </owl:DatatypeProperty>
  <owl:DatatypeProperty rdf:about="http://example.org/onto/prop/google_container_cluster_provisioned_iops">
    <rdfs:label>provisioned_iops</rdfs:label>
    <rdfs:comment>Configured IOPs provisioning. Only valid with disk type hyperdisk-balanced.</rdfs:comment>
    <rdfs:domain rdf:resource="http://example.org/onto/class/google_container_cluster"/>
    <rdfs:range rdf:resource="http://www.w3.org/2001/XMLSchema#string"/>
  </owl:DatatypeProperty>
  <owl:DatatypeProperty rdf:about="http://example.org/onto/prop/google_container_cluster_provisioned_throughput">
    <rdfs:label>provisioned_throughput</rdfs:label>
    <rdfs:comment>Configured throughput provisioning. Only valid with disk type hyperdisk-balanced.</rdfs:comment>
    <rdfs:domain rdf:resource="http://example.org/onto/class/google_container_cluster"/>
    <rdfs:range rdf:resource="http://www.w3.org/2001/XMLSchema#string"/>
  </owl:DatatypeProperty>
  <owl:DatatypeProperty rdf:about="http://example.org/onto/prop/google_container_cluster_size_gb">
    <rdfs:label>size_gb</rdfs:label>
    <rdfs:comment>Size of the disk attached to each node, specified in GB. The smallest allowed disk size is 10GB.</rdfs:comment>
    <rdfs:domain rdf:resource="http://example.org/onto/class/google_container_cluster"/>
    <rdfs:range rdf:resource="http://www.w3.org/2001/XMLSchema#string"/>
  </owl:DatatypeProperty>
  <owl:DatatypeProperty rdf:about="http://example.org/onto/prop/google_container_cluster_confidential_instance_type">
    <rdfs:label>confidential_instance_type</rdfs:label>
    <rdfs:comment>Defines the type of technology used by the confidential node.</rdfs:comment>
    <rdfs:domain rdf:resource="http://example.org/onto/class/google_container_cluster"/>
    <rdfs:range rdf:resource="http://www.w3.org/2001/XMLSchema#string"/>
  </owl:DatatypeProperty>
  <owl:DatatypeProperty rdf:about="http://example.org/onto/prop/google_container_cluster_enabled">
    <rdfs:label>enabled</rdfs:label>
    <rdfs:comment>Whether Confidential Nodes feature is enabled for all nodes in this pool.</rdfs:comment>
    <rdfs:domain rdf:resource="http://example.org/onto/class/google_container_cluster"/>
    <rdfs:range rdf:resource="http://www.w3.org/2001/XMLSchema#string"/>
  </owl:DatatypeProperty>
  <owl:DatatypeProperty rdf:about="http://example.org/onto/prop/google_container_cluster_enabled">
    <rdfs:label>enabled</rdfs:label>
    <rdfs:comment>Whether or not private registries are configured.</rdfs:comment>
    <rdfs:domain rdf:resource="http://example.org/onto/class/google_container_cluster"/>
    <rdfs:range rdf:resource="http://www.w3.org/2001/XMLSchema#string"/>
  </owl:DatatypeProperty>
  <owl:DatatypeProperty rdf:about="http://example.org/onto/prop/google_container_cluster_fqdns">
    <rdfs:label>fqdns</rdfs:label>
    <rdfs:comment>List of fully-qualified-domain-names. IPv4s and port specification are supported.</rdfs:comment>
    <rdfs:domain rdf:resource="http://example.org/onto/class/google_container_cluster"/>
    <rdfs:range rdf:resource="http://www.w3.org/2001/XMLSchema#string"/>
  </owl:DatatypeProperty>
  <owl:DatatypeProperty rdf:about="http://example.org/onto/prop/google_container_cluster_secret_uri">
    <rdfs:label>secret_uri</rdfs:label>
    <rdfs:comment>URI for the secret that hosts a certificate. Must be in the format 'projects/PROJECT_NUM/secrets/SECRET_NAME/versions/VERSION_OR_LATEST'.</rdfs:comment>
    <rdfs:domain rdf:resource="http://example.org/onto/class/google_container_cluster"/>
    <rdfs:range rdf:resource="http://www.w3.org/2001/XMLSchema#string"/>
  </owl:DatatypeProperty>
  <owl:DatatypeProperty rdf:about="http://example.org/onto/prop/google_container_cluster_data_cache_count">
    <rdfs:label>data_cache_count</rdfs:label>
    <rdfs:comment>Number of local SSDs to be utilized for GKE Data Cache. Uses NVMe interfaces.</rdfs:comment>
    <rdfs:domain rdf:resource="http://example.org/onto/class/google_container_cluster"/>
    <rdfs:range rdf:resource="http://www.w3.org/2001/XMLSchema#string"/>
  </owl:DatatypeProperty>
  <owl:DatatypeProperty rdf:about="http://example.org/onto/prop/google_container_cluster_local_ssd_count">
    <rdfs:label>local_ssd_count</rdfs:label>
    <rdfs:comment>Number of local SSDs to use to back ephemeral storage. Uses NVMe interfaces. Each local SSD must be 375 or 3000 GB in size, and all local SSDs must share the same size.</rdfs:comment>
    <rdfs:domain rdf:resource="http://example.org/onto/class/google_container_cluster"/>
    <rdfs:range rdf:resource="http://www.w3.org/2001/XMLSchema#string"/>
  </owl:DatatypeProperty>
  <owl:DatatypeProperty rdf:about="http://example.org/onto/prop/google_container_cluster_enabled">
    <rdfs:label>enabled</rdfs:label>
    <rdfs:comment>Whether or not NCCL Fast Socket is enabled</rdfs:comment>
    <rdfs:domain rdf:resource="http://example.org/onto/class/google_container_cluster"/>
    <rdfs:range rdf:resource="http://www.w3.org/2001/XMLSchema#string"/>
  </owl:DatatypeProperty>
  <owl:DatatypeProperty rdf:about="http://example.org/onto/prop/google_container_cluster_enabled">
    <rdfs:label>enabled</rdfs:label>
    <rdfs:comment>Whether or not GCFS is enabled</rdfs:comment>
    <rdfs:domain rdf:resource="http://example.org/onto/class/google_container_cluster"/>
    <rdfs:range rdf:resource="http://www.w3.org/2001/XMLSchema#string"/>
  </owl:DatatypeProperty>
  <owl:DatatypeProperty rdf:about="http://example.org/onto/prop/google_container_cluster_count">
    <rdfs:label>count</rdfs:label>
    <rdfs:comment>The number of the accelerator cards exposed to an instance.</rdfs:comment>
    <rdfs:domain rdf:resource="http://example.org/onto/class/google_container_cluster"/>
    <rdfs:range rdf:resource="http://www.w3.org/2001/XMLSchema#string"/>
  </owl:DatatypeProperty>
  <owl:DatatypeProperty rdf:about="http://example.org/onto/prop/google_container_cluster_gpu_partition_size">
    <rdfs:label>gpu_partition_size</rdfs:label>
    <rdfs:comment>Size of partitions to create on the GPU. Valid values are described in the NVIDIA mig user guide (https://docs.nvidia.com/datacenter/tesla/mig-user-guide/#partitioning)</rdfs:comment>
    <rdfs:domain rdf:resource="http://example.org/onto/class/google_container_cluster"/>
    <rdfs:range rdf:resource="http://www.w3.org/2001/XMLSchema#string"/>
  </owl:DatatypeProperty>
  <owl:DatatypeProperty rdf:about="http://example.org/onto/prop/google_container_cluster_type">
    <rdfs:label>type</rdfs:label>
    <rdfs:comment>The accelerator type resource name.</rdfs:comment>
    <rdfs:domain rdf:resource="http://example.org/onto/class/google_container_cluster"/>
    <rdfs:range rdf:resource="http://www.w3.org/2001/XMLSchema#string"/>
  </owl:DatatypeProperty>
  <owl:DatatypeProperty rdf:about="http://example.org/onto/prop/google_container_cluster_gpu_driver_version">
    <rdfs:label>gpu_driver_version</rdfs:label>
    <rdfs:comment>Mode for how the GPU driver is installed.</rdfs:comment>
    <rdfs:domain rdf:resource="http://example.org/onto/class/google_container_cluster"/>
    <rdfs:range rdf:resource="http://www.w3.org/2001/XMLSchema#string"/>
  </owl:DatatypeProperty>
  <owl:DatatypeProperty rdf:about="http://example.org/onto/prop/google_container_cluster_gpu_sharing_strategy">
    <rdfs:label>gpu_sharing_strategy</rdfs:label>
    <rdfs:comment>The type of GPU sharing strategy to enable on the GPU node. Possible values are described in the API package (https://pkg.go.dev/google.golang.org/api/container/v1#GPUSharingConfig)</rdfs:comment>
    <rdfs:domain rdf:resource="http://example.org/onto/class/google_container_cluster"/>
    <rdfs:range rdf:resource="http://www.w3.org/2001/XMLSchema#string"/>
  </owl:DatatypeProperty>
  <owl:DatatypeProperty rdf:about="http://example.org/onto/prop/google_container_cluster_max_shared_clients_per_gpu">
    <rdfs:label>max_shared_clients_per_gpu</rdfs:label>
    <rdfs:comment>The maximum number of containers that can share a GPU.</rdfs:comment>
    <rdfs:domain rdf:resource="http://example.org/onto/class/google_container_cluster"/>
    <rdfs:range rdf:resource="http://www.w3.org/2001/XMLSchema#string"/>
  </owl:DatatypeProperty>
  <owl:DatatypeProperty rdf:about="http://example.org/onto/prop/google_container_cluster_enabled">
    <rdfs:label>enabled</rdfs:label>
    <rdfs:comment>Whether or not gvnic is enabled</rdfs:comment>
    <rdfs:domain rdf:resource="http://example.org/onto/class/google_container_cluster"/>
    <rdfs:range rdf:resource="http://www.w3.org/2001/XMLSchema#string"/>
  </owl:DatatypeProperty>
  <owl:DatatypeProperty rdf:about="http://example.org/onto/prop/google_container_cluster_maintenance_interval">
    <rdfs:label>maintenance_interval</rdfs:label>
    <rdfs:comment>.</rdfs:comment>
    <rdfs:domain rdf:resource="http://example.org/onto/class/google_container_cluster"/>
    <rdfs:range rdf:resource="http://www.w3.org/2001/XMLSchema#string"/>
  </owl:DatatypeProperty>
  <owl:DatatypeProperty rdf:about="http://example.org/onto/prop/google_container_cluster_allowed_unsafe_sysctls">
    <rdfs:label>allowed_unsafe_sysctls</rdfs:label>
    <rdfs:comment>Defines a comma-separated allowlist of unsafe sysctls or sysctl patterns which can be set on the Pods.</rdfs:comment>
    <rdfs:domain rdf:resource="http://example.org/onto/class/google_container_cluster"/>
    <rdfs:range rdf:resource="http://www.w3.org/2001/XMLSchema#string"/>
  </owl:DatatypeProperty>
  <owl:DatatypeProperty rdf:about="http://example.org/onto/prop/google_container_cluster_container_log_max_files">
    <rdfs:label>container_log_max_files</rdfs:label>
    <rdfs:comment>Defines the maximum number of container log files that can be present for a container.</rdfs:comment>
    <rdfs:domain rdf:resource="http://example.org/onto/class/google_container_cluster"/>
    <rdfs:range rdf:resource="http://www.w3.org/2001/XMLSchema#string"/>
  </owl:DatatypeProperty>
  <owl:DatatypeProperty rdf:about="http://example.org/onto/prop/google_container_cluster_container_log_max_size">
    <rdfs:label>container_log_max_size</rdfs:label>
    <rdfs:comment>Defines the maximum size of the container log file before it is rotated.</rdfs:comment>
    <rdfs:domain rdf:resource="http://example.org/onto/class/google_container_cluster"/>
    <rdfs:range rdf:resource="http://www.w3.org/2001/XMLSchema#string"/>
  </owl:DatatypeProperty>
  <owl:DatatypeProperty rdf:about="http://example.org/onto/prop/google_container_cluster_cpu_cfs_quota">
    <rdfs:label>cpu_cfs_quota</rdfs:label>
    <rdfs:comment>Enable CPU CFS quota enforcement for containers that specify CPU limits.</rdfs:comment>
    <rdfs:domain rdf:resource="http://example.org/onto/class/google_container_cluster"/>
    <rdfs:range rdf:resource="http://www.w3.org/2001/XMLSchema#string"/>
  </owl:DatatypeProperty>
  <owl:DatatypeProperty rdf:about="http://example.org/onto/prop/google_container_cluster_cpu_cfs_quota_period">
    <rdfs:label>cpu_cfs_quota_period</rdfs:label>
    <rdfs:comment>Set the CPU CFS quota period value 'cpu.cfs_period_us'.</rdfs:comment>
    <rdfs:domain rdf:resource="http://example.org/onto/class/google_container_cluster"/>
    <rdfs:range rdf:resource="http://www.w3.org/2001/XMLSchema#string"/>
  </owl:DatatypeProperty>
  <owl:DatatypeProperty rdf:about="http://example.org/onto/prop/google_container_cluster_cpu_manager_policy">
    <rdfs:label>cpu_manager_policy</rdfs:label>
    <rdfs:comment>Control the CPU management policy on the node.</rdfs:comment>
    <rdfs:domain rdf:resource="http://example.org/onto/class/google_container_cluster"/>
    <rdfs:range rdf:resource="http://www.w3.org/2001/XMLSchema#string"/>
  </owl:DatatypeProperty>
  <owl:DatatypeProperty rdf:about="http://example.org/onto/prop/google_container_cluster_eviction_max_pod_grace_period_seconds">
    <rdfs:label>eviction_max_pod_grace_period_seconds</rdfs:label>
    <rdfs:comment>Defines the maximum allowed grace period (in seconds) to use when terminating pods in response to a soft eviction threshold being met.</rdfs:comment>
    <rdfs:domain rdf:resource="http://example.org/onto/class/google_container_cluster"/>
    <rdfs:range rdf:resource="http://www.w3.org/2001/XMLSchema#string"/>
  </owl:DatatypeProperty>
  <owl:DatatypeProperty rdf:about="http://example.org/onto/prop/google_container_cluster_image_gc_high_threshold_percent">
    <rdfs:label>image_gc_high_threshold_percent</rdfs:label>
    <rdfs:comment>Defines the percent of disk usage after which image garbage collection is always run.</rdfs:comment>
    <rdfs:domain rdf:resource="http://example.org/onto/class/google_container_cluster"/>
    <rdfs:range rdf:resource="http://www.w3.org/2001/XMLSchema#string"/>
  </owl:DatatypeProperty>
  <owl:DatatypeProperty rdf:about="http://example.org/onto/prop/google_container_cluster_image_gc_low_threshold_percent">
    <rdfs:label>image_gc_low_threshold_percent</rdfs:label>
    <rdfs:comment>Defines the percent of disk usage before which image garbage collection is never run. Lowest disk usage to garbage collect to.</rdfs:comment>
    <rdfs:domain rdf:resource="http://example.org/onto/class/google_container_cluster"/>
    <rdfs:range rdf:resource="http://www.w3.org/2001/XMLSchema#string"/>
  </owl:DatatypeProperty>
  <owl:DatatypeProperty rdf:about="http://example.org/onto/prop/google_container_cluster_image_maximum_gc_age">
    <rdfs:label>image_maximum_gc_age</rdfs:label>
    <rdfs:comment>Defines the maximum age an image can be unused before it is garbage collected.</rdfs:comment>
    <rdfs:domain rdf:resource="http://example.org/onto/class/google_container_cluster"/>
    <rdfs:range rdf:resource="http://www.w3.org/2001/XMLSchema#string"/>
  </owl:DatatypeProperty>
  <owl:DatatypeProperty rdf:about="http://example.org/onto/prop/google_container_cluster_image_minimum_gc_age">
    <rdfs:label>image_minimum_gc_age</rdfs:label>
    <rdfs:comment>Defines the minimum age for an unused image before it is garbage collected.</rdfs:comment>
    <rdfs:domain rdf:resource="http://example.org/onto/class/google_container_cluster"/>
    <rdfs:range rdf:resource="http://www.w3.org/2001/XMLSchema#string"/>
  </owl:DatatypeProperty>
  <owl:DatatypeProperty rdf:about="http://example.org/onto/prop/google_container_cluster_insecure_kubelet_readonly_port_enabled">
    <rdfs:label>insecure_kubelet_readonly_port_enabled</rdfs:label>
    <rdfs:comment>Controls whether the kubelet read-only port is enabled. It is strongly recommended to set this to `FALSE`. Possible values: `TRUE`, `FALSE`.</rdfs:comment>
    <rdfs:domain rdf:resource="http://example.org/onto/class/google_container_cluster"/>
    <rdfs:range rdf:resource="http://www.w3.org/2001/XMLSchema#string"/>
  </owl:DatatypeProperty>
  <owl:DatatypeProperty rdf:about="http://example.org/onto/prop/google_container_cluster_max_parallel_image_pulls">
    <rdfs:label>max_parallel_image_pulls</rdfs:label>
    <rdfs:comment>Set the maximum number of image pulls in parallel.</rdfs:comment>
    <rdfs:domain rdf:resource="http://example.org/onto/class/google_container_cluster"/>
    <rdfs:range rdf:resource="http://www.w3.org/2001/XMLSchema#string"/>
  </owl:DatatypeProperty>
  <owl:DatatypeProperty rdf:about="http://example.org/onto/prop/google_container_cluster_pod_pids_limit">
    <rdfs:label>pod_pids_limit</rdfs:label>
    <rdfs:comment>Controls the maximum number of processes allowed to run in a pod.</rdfs:comment>
    <rdfs:domain rdf:resource="http://example.org/onto/class/google_container_cluster"/>
    <rdfs:range rdf:resource="http://www.w3.org/2001/XMLSchema#string"/>
  </owl:DatatypeProperty>
  <owl:DatatypeProperty rdf:about="http://example.org/onto/prop/google_container_cluster_single_process_oom_kill">
    <rdfs:label>single_process_oom_kill</rdfs:label>
    <rdfs:comment>Defines whether to enable single process OOM killer.</rdfs:comment>
    <rdfs:domain rdf:resource="http://example.org/onto/class/google_container_cluster"/>
    <rdfs:range rdf:resource="http://www.w3.org/2001/XMLSchema#string"/>
  </owl:DatatypeProperty>
  <owl:DatatypeProperty rdf:about="http://example.org/onto/prop/google_container_cluster_imagefs_available">
    <rdfs:label>imagefs_available</rdfs:label>
    <rdfs:comment>Defines percentage of minimum reclaim for imagefs.available.</rdfs:comment>
    <rdfs:domain rdf:resource="http://example.org/onto/class/google_container_cluster"/>
    <rdfs:range rdf:resource="http://www.w3.org/2001/XMLSchema#string"/>
  </owl:DatatypeProperty>
  <owl:DatatypeProperty rdf:about="http://example.org/onto/prop/google_container_cluster_imagefs_inodes_free">
    <rdfs:label>imagefs_inodes_free</rdfs:label>
    <rdfs:comment>Defines percentage of minimum reclaim for imagefs.inodesFree.</rdfs:comment>
    <rdfs:domain rdf:resource="http://example.org/onto/class/google_container_cluster"/>
    <rdfs:range rdf:resource="http://www.w3.org/2001/XMLSchema#string"/>
  </owl:DatatypeProperty>
  <owl:DatatypeProperty rdf:about="http://example.org/onto/prop/google_container_cluster_memory_available">
    <rdfs:label>memory_available</rdfs:label>
    <rdfs:comment>Defines percentage of minimum reclaim for memory.available.</rdfs:comment>
    <rdfs:domain rdf:resource="http://example.org/onto/class/google_container_cluster"/>
    <rdfs:range rdf:resource="http://www.w3.org/2001/XMLSchema#string"/>
  </owl:DatatypeProperty>
  <owl:DatatypeProperty rdf:about="http://example.org/onto/prop/google_container_cluster_nodefs_available">
    <rdfs:label>nodefs_available</rdfs:label>
    <rdfs:comment>Defines percentage of minimum reclaim for nodefs.available.</rdfs:comment>
    <rdfs:domain rdf:resource="http://example.org/onto/class/google_container_cluster"/>
    <rdfs:range rdf:resource="http://www.w3.org/2001/XMLSchema#string"/>
  </owl:DatatypeProperty>
  <owl:DatatypeProperty rdf:about="http://example.org/onto/prop/google_container_cluster_nodefs_inodes_free">
    <rdfs:label>nodefs_inodes_free</rdfs:label>
    <rdfs:comment>Defines percentage of minimum reclaim for nodefs.inodesFree.</rdfs:comment>
    <rdfs:domain rdf:resource="http://example.org/onto/class/google_container_cluster"/>
    <rdfs:range rdf:resource="http://www.w3.org/2001/XMLSchema#string"/>
  </owl:DatatypeProperty>
  <owl:DatatypeProperty rdf:about="http://example.org/onto/prop/google_container_cluster_pid_available">
    <rdfs:label>pid_available</rdfs:label>
    <rdfs:comment>Defines percentage of minimum reclaim for pid.available.</rdfs:comment>
    <rdfs:domain rdf:resource="http://example.org/onto/class/google_container_cluster"/>
    <rdfs:range rdf:resource="http://www.w3.org/2001/XMLSchema#string"/>
  </owl:DatatypeProperty>
  <owl:DatatypeProperty rdf:about="http://example.org/onto/prop/google_container_cluster_imagefs_available">
    <rdfs:label>imagefs_available</rdfs:label>
    <rdfs:comment>Defines percentage of soft eviction threshold for imagefs.available.</rdfs:comment>
    <rdfs:domain rdf:resource="http://example.org/onto/class/google_container_cluster"/>
    <rdfs:range rdf:resource="http://www.w3.org/2001/XMLSchema#string"/>
  </owl:DatatypeProperty>
  <owl:DatatypeProperty rdf:about="http://example.org/onto/prop/google_container_cluster_imagefs_inodes_free">
    <rdfs:label>imagefs_inodes_free</rdfs:label>
    <rdfs:comment>Defines percentage of soft eviction threshold for imagefs.inodesFree.</rdfs:comment>
    <rdfs:domain rdf:resource="http://example.org/onto/class/google_container_cluster"/>
    <rdfs:range rdf:resource="http://www.w3.org/2001/XMLSchema#string"/>
  </owl:DatatypeProperty>
  <owl:DatatypeProperty rdf:about="http://example.org/onto/prop/google_container_cluster_memory_available">
    <rdfs:label>memory_available</rdfs:label>
    <rdfs:comment>Defines quantity of soft eviction threshold for memory.available.</rdfs:comment>
    <rdfs:domain rdf:resource="http://example.org/onto/class/google_container_cluster"/>
    <rdfs:range rdf:resource="http://www.w3.org/2001/XMLSchema#string"/>
  </owl:DatatypeProperty>
  <owl:DatatypeProperty rdf:about="http://example.org/onto/prop/google_container_cluster_nodefs_available">
    <rdfs:label>nodefs_available</rdfs:label>
    <rdfs:comment>Defines percentage of soft eviction threshold for nodefs.available.</rdfs:comment>
    <rdfs:domain rdf:resource="http://example.org/onto/class/google_container_cluster"/>
    <rdfs:range rdf:resource="http://www.w3.org/2001/XMLSchema#string"/>
  </owl:DatatypeProperty>
  <owl:DatatypeProperty rdf:about="http://example.org/onto/prop/google_container_cluster_nodefs_inodes_free">
    <rdfs:label>nodefs_inodes_free</rdfs:label>
    <rdfs:comment>Defines percentage of soft eviction threshold for nodefs.inodesFree.</rdfs:comment>
    <rdfs:domain rdf:resource="http://example.org/onto/class/google_container_cluster"/>
    <rdfs:range rdf:resource="http://www.w3.org/2001/XMLSchema#string"/>
  </owl:DatatypeProperty>
  <owl:DatatypeProperty rdf:about="http://example.org/onto/prop/google_container_cluster_pid_available">
    <rdfs:label>pid_available</rdfs:label>
    <rdfs:comment>Defines percentage of soft eviction threshold for pid.available.</rdfs:comment>
    <rdfs:domain rdf:resource="http://example.org/onto/class/google_container_cluster"/>
    <rdfs:range rdf:resource="http://www.w3.org/2001/XMLSchema#string"/>
  </owl:DatatypeProperty>
  <owl:DatatypeProperty rdf:about="http://example.org/onto/prop/google_container_cluster_imagefs_available">
    <rdfs:label>imagefs_available</rdfs:label>
    <rdfs:comment>Defines grace period for the imagefs.available soft eviction threshold</rdfs:comment>
    <rdfs:domain rdf:resource="http://example.org/onto/class/google_container_cluster"/>
    <rdfs:range rdf:resource="http://www.w3.org/2001/XMLSchema#string"/>
  </owl:DatatypeProperty>
  <owl:DatatypeProperty rdf:about="http://example.org/onto/prop/google_container_cluster_imagefs_inodes_free">
    <rdfs:label>imagefs_inodes_free</rdfs:label>
    <rdfs:comment>Defines grace period for the imagefs.inodesFree soft eviction threshold.</rdfs:comment>
    <rdfs:domain rdf:resource="http://example.org/onto/class/google_container_cluster"/>
    <rdfs:range rdf:resource="http://www.w3.org/2001/XMLSchema#string"/>
  </owl:DatatypeProperty>
  <owl:DatatypeProperty rdf:about="http://example.org/onto/prop/google_container_cluster_memory_available">
    <rdfs:label>memory_available</rdfs:label>
    <rdfs:comment>Defines grace period for the memory.available soft eviction threshold.</rdfs:comment>
    <rdfs:domain rdf:resource="http://example.org/onto/class/google_container_cluster"/>
    <rdfs:range rdf:resource="http://www.w3.org/2001/XMLSchema#string"/>
  </owl:DatatypeProperty>
  <owl:DatatypeProperty rdf:about="http://example.org/onto/prop/google_container_cluster_nodefs_available">
    <rdfs:label>nodefs_available</rdfs:label>
    <rdfs:comment>Defines grace period for the nodefs.available soft eviction threshold.</rdfs:comment>
    <rdfs:domain rdf:resource="http://example.org/onto/class/google_container_cluster"/>
    <rdfs:range rdf:resource="http://www.w3.org/2001/XMLSchema#string"/>
  </owl:DatatypeProperty>
  <owl:DatatypeProperty rdf:about="http://example.org/onto/prop/google_container_cluster_nodefs_inodes_free">
    <rdfs:label>nodefs_inodes_free</rdfs:label>
    <rdfs:comment>Defines grace period for the nodefs.inodesFree soft eviction threshold.</rdfs:comment>
    <rdfs:domain rdf:resource="http://example.org/onto/class/google_container_cluster"/>
    <rdfs:range rdf:resource="http://www.w3.org/2001/XMLSchema#string"/>
  </owl:DatatypeProperty>
  <owl:DatatypeProperty rdf:about="http://example.org/onto/prop/google_container_cluster_pid_available">
    <rdfs:label>pid_available</rdfs:label>
    <rdfs:comment>Defines grace period for the pid.available soft eviction threshold.</rdfs:comment>
    <rdfs:domain rdf:resource="http://example.org/onto/class/google_container_cluster"/>
    <rdfs:range rdf:resource="http://www.w3.org/2001/XMLSchema#string"/>
  </owl:DatatypeProperty>
  <owl:DatatypeProperty rdf:about="http://example.org/onto/prop/google_container_cluster_policy">
    <rdfs:label>policy</rdfs:label>
    <rdfs:comment>The Memory Manager policy to use. This policy guides how memory and hugepages are allocated and managed for pods on the node, influencing NUMA affinity.</rdfs:comment>
    <rdfs:domain rdf:resource="http://example.org/onto/class/google_container_cluster"/>
    <rdfs:range rdf:resource="http://www.w3.org/2001/XMLSchema#string"/>
  </owl:DatatypeProperty>
  <owl:DatatypeProperty rdf:about="http://example.org/onto/prop/google_container_cluster_policy">
    <rdfs:label>policy</rdfs:label>
    <rdfs:comment>The Topology Manager policy to use. This policy dictates how resource alignment is handled on the node.</rdfs:comment>
    <rdfs:domain rdf:resource="http://example.org/onto/class/google_container_cluster"/>
    <rdfs:range rdf:resource="http://www.w3.org/2001/XMLSchema#string"/>
  </owl:DatatypeProperty>
  <owl:DatatypeProperty rdf:about="http://example.org/onto/prop/google_container_cluster_scope">
    <rdfs:label>scope</rdfs:label>
    <rdfs:comment>The Topology Manager scope, defining the granularity at which policy decisions are applied. Valid values are "container" (resources are aligned per container within a pod) or "pod" (resources are aligned for the entire pod).</rdfs:comment>
    <rdfs:domain rdf:resource="http://example.org/onto/class/google_container_cluster"/>
    <rdfs:range rdf:resource="http://www.w3.org/2001/XMLSchema#string"/>
  </owl:DatatypeProperty>
  <owl:DatatypeProperty rdf:about="http://example.org/onto/prop/google_container_cluster_cgroup_mode">
    <rdfs:label>cgroup_mode</rdfs:label>
    <rdfs:comment>cgroupMode specifies the cgroup mode to be used on the node.</rdfs:comment>
    <rdfs:domain rdf:resource="http://example.org/onto/class/google_container_cluster"/>
    <rdfs:range rdf:resource="http://www.w3.org/2001/XMLSchema#string"/>
  </owl:DatatypeProperty>
  <owl:DatatypeProperty rdf:about="http://example.org/onto/prop/google_container_cluster_sysctls">
    <rdfs:label>sysctls</rdfs:label>
    <rdfs:comment>The Linux kernel parameters to be applied to the nodes and all pods running on the nodes.</rdfs:comment>
    <rdfs:domain rdf:resource="http://example.org/onto/class/google_container_cluster"/>
    <rdfs:range rdf:resource="http://www.w3.org/2001/XMLSchema#string"/>
  </owl:DatatypeProperty>
  <owl:DatatypeProperty rdf:about="http://example.org/onto/prop/google_container_cluster_transparent_hugepage_defrag">
    <rdfs:label>transparent_hugepage_defrag</rdfs:label>
    <rdfs:comment>The Linux kernel transparent hugepage defrag setting.</rdfs:comment>
    <rdfs:domain rdf:resource="http://example.org/onto/class/google_container_cluster"/>
    <rdfs:range rdf:resource="http://www.w3.org/2001/XMLSchema#string"/>
  </owl:DatatypeProperty>
  <owl:DatatypeProperty rdf:about="http://example.org/onto/prop/google_container_cluster_transparent_hugepage_enabled">
    <rdfs:label>transparent_hugepage_enabled</rdfs:label>
    <rdfs:comment>The Linux kernel transparent hugepage setting.</rdfs:comment>
    <rdfs:domain rdf:resource="http://example.org/onto/class/google_container_cluster"/>
    <rdfs:range rdf:resource="http://www.w3.org/2001/XMLSchema#string"/>
  </owl:DatatypeProperty>
  <owl:DatatypeProperty rdf:about="http://example.org/onto/prop/google_container_cluster_hugepage_size_1g">
    <rdfs:label>hugepage_size_1g</rdfs:label>
    <rdfs:comment>Amount of 1G hugepages.</rdfs:comment>
    <rdfs:domain rdf:resource="http://example.org/onto/class/google_container_cluster"/>
    <rdfs:range rdf:resource="http://www.w3.org/2001/XMLSchema#string"/>
  </owl:DatatypeProperty>
  <owl:DatatypeProperty rdf:about="http://example.org/onto/prop/google_container_cluster_hugepage_size_2m">
    <rdfs:label>hugepage_size_2m</rdfs:label>
    <rdfs:comment>Amount of 2M hugepages.</rdfs:comment>
    <rdfs:domain rdf:resource="http://example.org/onto/class/google_container_cluster"/>
    <rdfs:range rdf:resource="http://www.w3.org/2001/XMLSchema#string"/>
  </owl:DatatypeProperty>
  <owl:DatatypeProperty rdf:about="http://example.org/onto/prop/google_container_cluster_local_ssd_count">
    <rdfs:label>local_ssd_count</rdfs:label>
    <rdfs:comment>Number of raw-block local NVMe SSD disks to be attached to the node. Each local SSD is 375 GB in size.</rdfs:comment>
    <rdfs:domain rdf:resource="http://example.org/onto/class/google_container_cluster"/>
    <rdfs:range rdf:resource="http://www.w3.org/2001/XMLSchema#string"/>
  </owl:DatatypeProperty>
  <owl:DatatypeProperty rdf:about="http://example.org/onto/prop/google_container_cluster_consume_reservation_type">
    <rdfs:label>consume_reservation_type</rdfs:label>
    <rdfs:comment>Corresponds to the type of reservation consumption.</rdfs:comment>
    <rdfs:domain rdf:resource="http://example.org/onto/class/google_container_cluster"/>
    <rdfs:range rdf:resource="http://www.w3.org/2001/XMLSchema#string"/>
  </owl:DatatypeProperty>
  <owl:DatatypeProperty rdf:about="http://example.org/onto/prop/google_container_cluster_key">
    <rdfs:label>key</rdfs:label>
    <rdfs:comment>The label key of a reservation resource.</rdfs:comment>
    <rdfs:domain rdf:resource="http://example.org/onto/class/google_container_cluster"/>
    <rdfs:range rdf:resource="http://www.w3.org/2001/XMLSchema#string"/>
  </owl:DatatypeProperty>
  <owl:DatatypeProperty rdf:about="http://example.org/onto/prop/google_container_cluster_values">
    <rdfs:label>values</rdfs:label>
    <rdfs:comment>The label values of the reservation resource.</rdfs:comment>
    <rdfs:domain rdf:resource="http://example.org/onto/class/google_container_cluster"/>
    <rdfs:range rdf:resource="http://www.w3.org/2001/XMLSchema#string"/>
  </owl:DatatypeProperty>
  <owl:DatatypeProperty rdf:about="http://example.org/onto/prop/google_container_cluster_disk_image">
    <rdfs:label>disk_image</rdfs:label>
    <rdfs:comment>Disk image to create the secondary boot disk from</rdfs:comment>
    <rdfs:domain rdf:resource="http://example.org/onto/class/google_container_cluster"/>
    <rdfs:range rdf:resource="http://www.w3.org/2001/XMLSchema#string"/>
  </owl:DatatypeProperty>
  <owl:DatatypeProperty rdf:about="http://example.org/onto/prop/google_container_cluster_mode">
    <rdfs:label>mode</rdfs:label>
    <rdfs:comment>Mode for how the secondary boot disk is used.</rdfs:comment>
    <rdfs:domain rdf:resource="http://example.org/onto/class/google_container_cluster"/>
    <rdfs:range rdf:resource="http://www.w3.org/2001/XMLSchema#string"/>
  </owl:DatatypeProperty>
  <owl:DatatypeProperty rdf:about="http://example.org/onto/prop/google_container_cluster_enable_integrity_monitoring">
    <rdfs:label>enable_integrity_monitoring</rdfs:label>
    <rdfs:comment>Defines whether the instance has integrity monitoring enabled.</rdfs:comment>
    <rdfs:domain rdf:resource="http://example.org/onto/class/google_container_cluster"/>
    <rdfs:range rdf:resource="http://www.w3.org/2001/XMLSchema#string"/>
  </owl:DatatypeProperty>
  <owl:DatatypeProperty rdf:about="http://example.org/onto/prop/google_container_cluster_enable_secure_boot">
    <rdfs:label>enable_secure_boot</rdfs:label>
    <rdfs:comment>Defines whether the instance has Secure Boot enabled.</rdfs:comment>
    <rdfs:domain rdf:resource="http://example.org/onto/class/google_container_cluster"/>
    <rdfs:range rdf:resource="http://www.w3.org/2001/XMLSchema#string"/>
  </owl:DatatypeProperty>
  <owl:DatatypeProperty rdf:about="http://example.org/onto/prop/google_container_cluster_min_node_cpus">
    <rdfs:label>min_node_cpus</rdfs:label>
    <rdfs:comment>Specifies the minimum number of vCPUs that each sole tenant node must have to use CPU overcommit. If not specified, the CPU overcommit feature is disabled.</rdfs:comment>
    <rdfs:domain rdf:resource="http://example.org/onto/class/google_container_cluster"/>
    <rdfs:range rdf:resource="http://www.w3.org/2001/XMLSchema#string"/>
  </owl:DatatypeProperty>
  <owl:DatatypeProperty rdf:about="http://example.org/onto/prop/google_container_cluster_key">
    <rdfs:label>key</rdfs:label>
    <rdfs:comment>.</rdfs:comment>
    <rdfs:domain rdf:resource="http://example.org/onto/class/google_container_cluster"/>
    <rdfs:range rdf:resource="http://www.w3.org/2001/XMLSchema#string"/>
  </owl:DatatypeProperty>
  <owl:DatatypeProperty rdf:about="http://example.org/onto/prop/google_container_cluster_operator">
    <rdfs:label>operator</rdfs:label>
    <rdfs:comment>.</rdfs:comment>
    <rdfs:domain rdf:resource="http://example.org/onto/class/google_container_cluster"/>
    <rdfs:range rdf:resource="http://www.w3.org/2001/XMLSchema#string"/>
  </owl:DatatypeProperty>
  <owl:DatatypeProperty rdf:about="http://example.org/onto/prop/google_container_cluster_values">
    <rdfs:label>values</rdfs:label>
    <rdfs:comment>.</rdfs:comment>
    <rdfs:domain rdf:resource="http://example.org/onto/class/google_container_cluster"/>
    <rdfs:range rdf:resource="http://www.w3.org/2001/XMLSchema#string"/>
  </owl:DatatypeProperty>
  <owl:DatatypeProperty rdf:about="http://example.org/onto/prop/google_container_cluster_effect">
    <rdfs:label>effect</rdfs:label>
    <rdfs:comment>Effect for taint.</rdfs:comment>
    <rdfs:domain rdf:resource="http://example.org/onto/class/google_container_cluster"/>
    <rdfs:range rdf:resource="http://www.w3.org/2001/XMLSchema#string"/>
  </owl:DatatypeProperty>
  <owl:DatatypeProperty rdf:about="http://example.org/onto/prop/google_container_cluster_key">
    <rdfs:label>key</rdfs:label>
    <rdfs:comment>Key for taint.</rdfs:comment>
    <rdfs:domain rdf:resource="http://example.org/onto/class/google_container_cluster"/>
    <rdfs:range rdf:resource="http://www.w3.org/2001/XMLSchema#string"/>
  </owl:DatatypeProperty>
  <owl:DatatypeProperty rdf:about="http://example.org/onto/prop/google_container_cluster_value">
    <rdfs:label>value</rdfs:label>
    <rdfs:comment>Value for taint.</rdfs:comment>
    <rdfs:domain rdf:resource="http://example.org/onto/class/google_container_cluster"/>
    <rdfs:range rdf:resource="http://www.w3.org/2001/XMLSchema#string"/>
  </owl:DatatypeProperty>
  <owl:DatatypeProperty rdf:about="http://example.org/onto/prop/google_container_cluster_osversion">
    <rdfs:label>osversion</rdfs:label>
    <rdfs:comment>The OS Version of the windows nodepool.Values are OS_VERSION_UNSPECIFIED,OS_VERSION_LTSC2019 and OS_VERSION_LTSC2022</rdfs:comment>
    <rdfs:domain rdf:resource="http://example.org/onto/class/google_container_cluster"/>
    <rdfs:range rdf:resource="http://www.w3.org/2001/XMLSchema#string"/>
  </owl:DatatypeProperty>
  <owl:DatatypeProperty rdf:about="http://example.org/onto/prop/google_container_cluster_mode">
    <rdfs:label>mode</rdfs:label>
    <rdfs:comment>Mode is the configuration for how to expose metadata to workloads running on the node.</rdfs:comment>
    <rdfs:domain rdf:resource="http://example.org/onto/class/google_container_cluster"/>
    <rdfs:range rdf:resource="http://www.w3.org/2001/XMLSchema#string"/>
  </owl:DatatypeProperty>
  <owl:DatatypeProperty rdf:about="http://example.org/onto/prop/google_container_cluster_policy_name">
    <rdfs:label>policy_name</rdfs:label>
    <rdfs:comment>If set, refers to the name of a custom resource policy supplied by the user. The resource policy must be in the same project and region as the node pool. If not found, InvalidArgument error is returned.</rdfs:comment>
    <rdfs:domain rdf:resource="http://example.org/onto/class/google_container_cluster"/>
    <rdfs:range rdf:resource="http://www.w3.org/2001/XMLSchema#string"/>
  </owl:DatatypeProperty>
  <owl:DatatypeProperty rdf:about="http://example.org/onto/prop/google_container_cluster_tpu_topology">
    <rdfs:label>tpu_topology</rdfs:label>
    <rdfs:comment>The TPU topology like "2x4" or "2x2x2". https://cloud.google.com/kubernetes-engine/docs/concepts/plan-tpus#topology</rdfs:comment>
    <rdfs:domain rdf:resource="http://example.org/onto/class/google_container_cluster"/>
    <rdfs:range rdf:resource="http://www.w3.org/2001/XMLSchema#string"/>
  </owl:DatatypeProperty>
  <owl:DatatypeProperty rdf:about="http://example.org/onto/prop/google_container_cluster_type">
    <rdfs:label>type</rdfs:label>
    <rdfs:comment>Type defines the type of placement policy</rdfs:comment>
    <rdfs:domain rdf:resource="http://example.org/onto/class/google_container_cluster"/>
    <rdfs:range rdf:resource="http://www.w3.org/2001/XMLSchema#string"/>
  </owl:DatatypeProperty>
  <owl:DatatypeProperty rdf:about="http://example.org/onto/prop/google_container_cluster_enabled">
    <rdfs:label>enabled</rdfs:label>
    <rdfs:comment>Whether nodes in this node pool are obtainable solely through the ProvisioningRequest API</rdfs:comment>
    <rdfs:domain rdf:resource="http://example.org/onto/class/google_container_cluster"/>
    <rdfs:range rdf:resource="http://www.w3.org/2001/XMLSchema#string"/>
  </owl:DatatypeProperty>
  <owl:DatatypeProperty rdf:about="http://example.org/onto/prop/google_container_cluster_max_surge">
    <rdfs:label>max_surge</rdfs:label>
    <rdfs:comment>The number of additional nodes that can be added to the node pool during an upgrade. Increasing max_surge raises the number of nodes that can be upgraded simultaneously. Can be set to 0 or greater.</rdfs:comment>
    <rdfs:domain rdf:resource="http://example.org/onto/class/google_container_cluster"/>
    <rdfs:range rdf:resource="http://www.w3.org/2001/XMLSchema#string"/>
  </owl:DatatypeProperty>
  <owl:DatatypeProperty rdf:about="http://example.org/onto/prop/google_container_cluster_max_unavailable">
    <rdfs:label>max_unavailable</rdfs:label>
    <rdfs:comment>The number of nodes that can be simultaneously unavailable during an upgrade. Increasing max_unavailable raises the number of nodes that can be upgraded in parallel. Can be set to 0 or greater.</rdfs:comment>
    <rdfs:domain rdf:resource="http://example.org/onto/class/google_container_cluster"/>
    <rdfs:range rdf:resource="http://www.w3.org/2001/XMLSchema#string"/>
  </owl:DatatypeProperty>
  <owl:DatatypeProperty rdf:about="http://example.org/onto/prop/google_container_cluster_strategy">
    <rdfs:label>strategy</rdfs:label>
    <rdfs:comment>Update strategy for the given nodepool.</rdfs:comment>
    <rdfs:domain rdf:resource="http://example.org/onto/class/google_container_cluster"/>
    <rdfs:range rdf:resource="http://www.w3.org/2001/XMLSchema#string"/>
  </owl:DatatypeProperty>
  <owl:DatatypeProperty rdf:about="http://example.org/onto/prop/google_container_cluster_node_pool_soak_duration">
    <rdfs:label>node_pool_soak_duration</rdfs:label>
    <rdfs:comment>Time needed after draining entire blue pool. After this period, blue pool will be cleaned up.</rdfs:comment>
    <rdfs:domain rdf:resource="http://example.org/onto/class/google_container_cluster"/>
    <rdfs:range rdf:resource="http://www.w3.org/2001/XMLSchema#string"/>
  </owl:DatatypeProperty>
  <owl:DatatypeProperty rdf:about="http://example.org/onto/prop/google_container_cluster_batch_node_count">
    <rdfs:label>batch_node_count</rdfs:label>
    <rdfs:comment>Number of blue nodes to drain in a batch.</rdfs:comment>
    <rdfs:domain rdf:resource="http://example.org/onto/class/google_container_cluster"/>
    <rdfs:range rdf:resource="http://www.w3.org/2001/XMLSchema#string"/>
  </owl:DatatypeProperty>
  <owl:DatatypeProperty rdf:about="http://example.org/onto/prop/google_container_cluster_batch_percentage">
    <rdfs:label>batch_percentage</rdfs:label>
    <rdfs:comment>Percentage of the blue pool nodes to drain in a batch.</rdfs:comment>
    <rdfs:domain rdf:resource="http://example.org/onto/class/google_container_cluster"/>
    <rdfs:range rdf:resource="http://www.w3.org/2001/XMLSchema#string"/>
  </owl:DatatypeProperty>
  <owl:DatatypeProperty rdf:about="http://example.org/onto/prop/google_container_cluster_batch_soak_duration">
    <rdfs:label>batch_soak_duration</rdfs:label>
    <rdfs:comment>Soak time after each batch gets drained.</rdfs:comment>
    <rdfs:domain rdf:resource="http://example.org/onto/class/google_container_cluster"/>
    <rdfs:range rdf:resource="http://www.w3.org/2001/XMLSchema#string"/>
  </owl:DatatypeProperty>
  <owl:DatatypeProperty rdf:about="http://example.org/onto/prop/google_container_cluster_resource_manager_tags">
    <rdfs:label>resource_manager_tags</rdfs:label>
    <rdfs:comment>A map of resource manager tags. Resource manager tag keys and values have the same definition as resource manager tags. Keys must be in the format tagKeys/{tag_key_id}, and values are in the format tagValues/456. The field is ignored (both PUT & PATCH) when empty.</rdfs:comment>
    <rdfs:domain rdf:resource="http://example.org/onto/class/google_container_cluster"/>
    <rdfs:range rdf:resource="http://www.w3.org/2001/XMLSchema#string"/>
  </owl:DatatypeProperty>
  <owl:DatatypeProperty rdf:about="http://example.org/onto/prop/google_container_cluster_cgroup_mode">
    <rdfs:label>cgroup_mode</rdfs:label>
    <rdfs:comment>cgroupMode specifies the cgroup mode to be used on the node.</rdfs:comment>
    <rdfs:domain rdf:resource="http://example.org/onto/class/google_container_cluster"/>
    <rdfs:range rdf:resource="http://www.w3.org/2001/XMLSchema#string"/>
  </owl:DatatypeProperty>
  <owl:DatatypeProperty rdf:about="http://example.org/onto/prop/google_container_cluster_tags">
    <rdfs:label>tags</rdfs:label>
    <rdfs:comment>List of network tags applied to auto-provisioned node pools.</rdfs:comment>
    <rdfs:domain rdf:resource="http://example.org/onto/class/google_container_cluster"/>
    <rdfs:range rdf:resource="http://www.w3.org/2001/XMLSchema#string"/>
  </owl:DatatypeProperty>
  <owl:DatatypeProperty rdf:about="http://example.org/onto/prop/google_container_cluster_insecure_kubelet_readonly_port_enabled">
    <rdfs:label>insecure_kubelet_readonly_port_enabled</rdfs:label>
    <rdfs:comment>Controls whether the kubelet read-only port is enabled. It is strongly recommended to set this to `FALSE`. Possible values: `TRUE`, `FALSE`.</rdfs:comment>
    <rdfs:domain rdf:resource="http://example.org/onto/class/google_container_cluster"/>
    <rdfs:range rdf:resource="http://www.w3.org/2001/XMLSchema#string"/>
  </owl:DatatypeProperty>
  <owl:DatatypeProperty rdf:about="http://example.org/onto/prop/google_container_cluster_insecure_kubelet_readonly_port_enabled">
    <rdfs:label>insecure_kubelet_readonly_port_enabled</rdfs:label>
    <rdfs:comment>Controls whether the kubelet read-only port is enabled. It is strongly recommended to set this to `FALSE`. Possible values: `TRUE`, `FALSE`.</rdfs:comment>
    <rdfs:domain rdf:resource="http://example.org/onto/class/google_container_cluster"/>
    <rdfs:range rdf:resource="http://www.w3.org/2001/XMLSchema#string"/>
  </owl:DatatypeProperty>
  <owl:DatatypeProperty rdf:about="http://example.org/onto/prop/google_container_cluster_logging_variant">
    <rdfs:label>logging_variant</rdfs:label>
    <rdfs:comment>Type of logging agent that is used as the default value for node pools in the cluster. Valid values include DEFAULT and MAX_THROUGHPUT.</rdfs:comment>
    <rdfs:domain rdf:resource="http://example.org/onto/class/google_container_cluster"/>
    <rdfs:range rdf:resource="http://www.w3.org/2001/XMLSchema#string"/>
  </owl:DatatypeProperty>
  <owl:DatatypeProperty rdf:about="http://example.org/onto/prop/google_container_cluster_enabled">
    <rdfs:label>enabled</rdfs:label>
    <rdfs:comment>Whether or not private registries are configured.</rdfs:comment>
    <rdfs:domain rdf:resource="http://example.org/onto/class/google_container_cluster"/>
    <rdfs:range rdf:resource="http://www.w3.org/2001/XMLSchema#string"/>
  </owl:DatatypeProperty>
  <owl:DatatypeProperty rdf:about="http://example.org/onto/prop/google_container_cluster_fqdns">
    <rdfs:label>fqdns</rdfs:label>
    <rdfs:comment>List of fully-qualified-domain-names. IPv4s and port specification are supported.</rdfs:comment>
    <rdfs:domain rdf:resource="http://example.org/onto/class/google_container_cluster"/>
    <rdfs:range rdf:resource="http://www.w3.org/2001/XMLSchema#string"/>
  </owl:DatatypeProperty>
  <owl:DatatypeProperty rdf:about="http://example.org/onto/prop/google_container_cluster_secret_uri">
    <rdfs:label>secret_uri</rdfs:label>
    <rdfs:comment>URI for the secret that hosts a certificate. Must be in the format 'projects/PROJECT_NUM/secrets/SECRET_NAME/versions/VERSION_OR_LATEST'.</rdfs:comment>
    <rdfs:domain rdf:resource="http://example.org/onto/class/google_container_cluster"/>
    <rdfs:range rdf:resource="http://www.w3.org/2001/XMLSchema#string"/>
  </owl:DatatypeProperty>
  <owl:DatatypeProperty rdf:about="http://example.org/onto/prop/google_container_cluster_enabled">
    <rdfs:label>enabled</rdfs:label>
    <rdfs:comment>Whether or not GCFS is enabled</rdfs:comment>
    <rdfs:domain rdf:resource="http://example.org/onto/class/google_container_cluster"/>
    <rdfs:range rdf:resource="http://www.w3.org/2001/XMLSchema#string"/>
  </owl:DatatypeProperty>
  <owl:DatatypeProperty rdf:about="http://example.org/onto/prop/google_container_cluster_enabled">
    <rdfs:label>enabled</rdfs:label>
    <rdfs:comment>Whether or not the notification config is enabled</rdfs:comment>
    <rdfs:domain rdf:resource="http://example.org/onto/class/google_container_cluster"/>
    <rdfs:range rdf:resource="http://www.w3.org/2001/XMLSchema#string"/>
  </owl:DatatypeProperty>
  <owl:DatatypeProperty rdf:about="http://example.org/onto/prop/google_container_cluster_topic">
    <rdfs:label>topic</rdfs:label>
    <rdfs:comment>The pubsub topic to push upgrade notifications to. Must be in the same project as the cluster. Must be in the format: projects/{project}/topics/{topic}.</rdfs:comment>
    <rdfs:domain rdf:resource="http://example.org/onto/class/google_container_cluster"/>
    <rdfs:range rdf:resource="http://www.w3.org/2001/XMLSchema#string"/>
  </owl:DatatypeProperty>
  <owl:DatatypeProperty rdf:about="http://example.org/onto/prop/google_container_cluster_event_type">
    <rdfs:label>event_type</rdfs:label>
    <rdfs:comment>Can be used to filter what notifications are sent. Valid values include include UPGRADE_AVAILABLE_EVENT, UPGRADE_EVENT, SECURITY_BULLETIN_EVENT, and UPGRADE_INFO_EVENT</rdfs:comment>
    <rdfs:domain rdf:resource="http://example.org/onto/class/google_container_cluster"/>
    <rdfs:range rdf:resource="http://www.w3.org/2001/XMLSchema#string"/>
  </owl:DatatypeProperty>
  <owl:DatatypeProperty rdf:about="http://example.org/onto/prop/google_container_cluster_hpa_profile">
    <rdfs:label>hpa_profile</rdfs:label>
    <rdfs:comment>HPA Profile is used to configure the Horizontal Pod Autoscaler (HPA) profile for the cluster.
								Available options include:
								- NONE: Customers explicitly opt-out of HPA profiles.
								- PERFORMANCE: PERFORMANCE is used when customers opt-in to the performance HPA profile. In this profile we support a higher number of HPAs per cluster and faster metrics collection for workload autoscaling.</rdfs:comment>
    <rdfs:domain rdf:resource="http://example.org/onto/class/google_container_cluster"/>
    <rdfs:range rdf:resource="http://www.w3.org/2001/XMLSchema#string"/>
  </owl:DatatypeProperty>
  <owl:DatatypeProperty rdf:about="http://example.org/onto/prop/google_container_cluster_enable_private_endpoint">
    <rdfs:label>enable_private_endpoint</rdfs:label>
    <rdfs:comment>When true, the cluster's private endpoint is used as the cluster endpoint and access through the public endpoint is disabled. When false, either endpoint can be used.</rdfs:comment>
    <rdfs:domain rdf:resource="http://example.org/onto/class/google_container_cluster"/>
    <rdfs:range rdf:resource="http://www.w3.org/2001/XMLSchema#string"/>
  </owl:DatatypeProperty>
  <owl:DatatypeProperty rdf:about="http://example.org/onto/prop/google_container_cluster_enable_private_nodes">
    <rdfs:label>enable_private_nodes</rdfs:label>
    <rdfs:comment>Enables the private cluster feature, creating a private endpoint on the cluster. In a private cluster, nodes only have RFC 1918 private addresses and communicate with the master's private endpoint via private networking.</rdfs:comment>
    <rdfs:domain rdf:resource="http://example.org/onto/class/google_container_cluster"/>
    <rdfs:range rdf:resource="http://www.w3.org/2001/XMLSchema#string"/>
  </owl:DatatypeProperty>
  <owl:DatatypeProperty rdf:about="http://example.org/onto/prop/google_container_cluster_master_ipv4_cidr_block">
    <rdfs:label>master_ipv4_cidr_block</rdfs:label>
    <rdfs:comment>The IP range in CIDR notation to use for the hosted master network. This range will be used for assigning private IP addresses to the cluster master(s) and the ILB VIP. This range must not overlap with any other ranges in use within the cluster's network, and it must be a /28 subnet. See Private Cluster Limitations for more details. This field only applies to private clusters, when enable_private_nodes is true.</rdfs:comment>
    <rdfs:domain rdf:resource="http://example.org/onto/class/google_container_cluster"/>
    <rdfs:range rdf:resource="http://www.w3.org/2001/XMLSchema#string"/>
  </owl:DatatypeProperty>
  <owl:DatatypeProperty rdf:about="http://example.org/onto/prop/google_container_cluster_peering_name">
    <rdfs:label>peering_name</rdfs:label>
    <rdfs:comment>The name of the peering between this cluster and the Google owned VPC.</rdfs:comment>
    <rdfs:domain rdf:resource="http://example.org/onto/class/google_container_cluster"/>
    <rdfs:range rdf:resource="http://www.w3.org/2001/XMLSchema#string"/>
  </owl:DatatypeProperty>
  <owl:DatatypeProperty rdf:about="http://example.org/onto/prop/google_container_cluster_private_endpoint">
    <rdfs:label>private_endpoint</rdfs:label>
    <rdfs:comment>The internal IP address of this cluster's master endpoint.</rdfs:comment>
    <rdfs:domain rdf:resource="http://example.org/onto/class/google_container_cluster"/>
    <rdfs:range rdf:resource="http://www.w3.org/2001/XMLSchema#string"/>
  </owl:DatatypeProperty>
  <owl:DatatypeProperty rdf:about="http://example.org/onto/prop/google_container_cluster_private_endpoint_subnetwork">
    <rdfs:label>private_endpoint_subnetwork</rdfs:label>
    <rdfs:comment>Subnetwork in cluster's network where master's endpoint will be provisioned.</rdfs:comment>
    <rdfs:domain rdf:resource="http://example.org/onto/class/google_container_cluster"/>
    <rdfs:range rdf:resource="http://www.w3.org/2001/XMLSchema#string"/>
  </owl:DatatypeProperty>
  <owl:DatatypeProperty rdf:about="http://example.org/onto/prop/google_container_cluster_public_endpoint">
    <rdfs:label>public_endpoint</rdfs:label>
    <rdfs:comment>The external IP address of this cluster's master endpoint.</rdfs:comment>
    <rdfs:domain rdf:resource="http://example.org/onto/class/google_container_cluster"/>
    <rdfs:range rdf:resource="http://www.w3.org/2001/XMLSchema#string"/>
  </owl:DatatypeProperty>
  <owl:DatatypeProperty rdf:about="http://example.org/onto/prop/google_container_cluster_enabled">
    <rdfs:label>enabled</rdfs:label>
    <rdfs:comment>Whether the cluster master is accessible globally or not.</rdfs:comment>
    <rdfs:domain rdf:resource="http://example.org/onto/class/google_container_cluster"/>
    <rdfs:range rdf:resource="http://www.w3.org/2001/XMLSchema#string"/>
  </owl:DatatypeProperty>
  <owl:DatatypeProperty rdf:about="http://example.org/onto/prop/google_container_cluster_enable_insecure_binding_system_authenticated">
    <rdfs:label>enable_insecure_binding_system_authenticated</rdfs:label>
    <rdfs:comment>Setting this to true will allow any ClusterRoleBinding and RoleBinding with subjects system:authenticated.</rdfs:comment>
    <rdfs:domain rdf:resource="http://example.org/onto/class/google_container_cluster"/>
    <rdfs:range rdf:resource="http://www.w3.org/2001/XMLSchema#string"/>
  </owl:DatatypeProperty>
  <owl:DatatypeProperty rdf:about="http://example.org/onto/prop/google_container_cluster_enable_insecure_binding_system_unauthenticated">
    <rdfs:label>enable_insecure_binding_system_unauthenticated</rdfs:label>
    <rdfs:comment>Setting this to true will allow any ClusterRoleBinding and RoleBinding with subjects system:anonymous or system:unauthenticated.</rdfs:comment>
    <rdfs:domain rdf:resource="http://example.org/onto/class/google_container_cluster"/>
    <rdfs:range rdf:resource="http://www.w3.org/2001/XMLSchema#string"/>
  </owl:DatatypeProperty>
  <owl:DatatypeProperty rdf:about="http://example.org/onto/prop/google_container_cluster_channel">
    <rdfs:label>channel</rdfs:label>
    <rdfs:comment>The selected release channel. Accepted values are:
* UNSPECIFIED: Not set.
* RAPID: Weekly upgrade cadence; Early testers and developers who requires new features.
* REGULAR: Multiple per month upgrade cadence; Production users who need features not yet offered in the Stable channel.
* STABLE: Every few months upgrade cadence; Production users who need stability above all else, and for whom frequent upgrades are too risky.
* EXTENDED: GKE provides extended support for Kubernetes minor versions through the Extended channel. With this channel, you can stay on a minor version for up to 24 months.</rdfs:comment>
    <rdfs:domain rdf:resource="http://example.org/onto/class/google_container_cluster"/>
    <rdfs:range rdf:resource="http://www.w3.org/2001/XMLSchema#string"/>
  </owl:DatatypeProperty>
  <owl:DatatypeProperty rdf:about="http://example.org/onto/prop/google_container_cluster_enable_network_egress_metering">
    <rdfs:label>enable_network_egress_metering</rdfs:label>
    <rdfs:comment>Whether to enable network egress metering for this cluster. If enabled, a daemonset will be created in the cluster to meter network egress traffic.</rdfs:comment>
    <rdfs:domain rdf:resource="http://example.org/onto/class/google_container_cluster"/>
    <rdfs:range rdf:resource="http://www.w3.org/2001/XMLSchema#string"/>
  </owl:DatatypeProperty>
  <owl:DatatypeProperty rdf:about="http://example.org/onto/prop/google_container_cluster_enable_resource_consumption_metering">
    <rdfs:label>enable_resource_consumption_metering</rdfs:label>
    <rdfs:comment>Whether to enable resource consumption metering on this cluster. When enabled, a table will be created in the resource export BigQuery dataset to store resource consumption data. The resulting table can be joined with the resource usage table or with BigQuery billing export. Defaults to true.</rdfs:comment>
    <rdfs:domain rdf:resource="http://example.org/onto/class/google_container_cluster"/>
    <rdfs:range rdf:resource="http://www.w3.org/2001/XMLSchema#string"/>
  </owl:DatatypeProperty>
  <owl:DatatypeProperty rdf:about="http://example.org/onto/prop/google_container_cluster_dataset_id">
    <rdfs:label>dataset_id</rdfs:label>
    <rdfs:comment>The ID of a BigQuery Dataset.</rdfs:comment>
    <rdfs:domain rdf:resource="http://example.org/onto/class/google_container_cluster"/>
    <rdfs:range rdf:resource="http://www.w3.org/2001/XMLSchema#string"/>
  </owl:DatatypeProperty>
  <owl:DatatypeProperty rdf:about="http://example.org/onto/prop/google_container_cluster_enabled">
    <rdfs:label>enabled</rdfs:label>
    <rdfs:comment>Enable the Secret manager csi component.</rdfs:comment>
    <rdfs:domain rdf:resource="http://example.org/onto/class/google_container_cluster"/>
    <rdfs:range rdf:resource="http://www.w3.org/2001/XMLSchema#string"/>
  </owl:DatatypeProperty>
  <owl:DatatypeProperty rdf:about="http://example.org/onto/prop/google_container_cluster_enabled">
    <rdfs:label>enabled</rdfs:label>
    <rdfs:comment>Enable the Secret manager auto rotation.</rdfs:comment>
    <rdfs:domain rdf:resource="http://example.org/onto/class/google_container_cluster"/>
    <rdfs:range rdf:resource="http://www.w3.org/2001/XMLSchema#string"/>
  </owl:DatatypeProperty>
  <owl:DatatypeProperty rdf:about="http://example.org/onto/prop/google_container_cluster_rotation_interval">
    <rdfs:label>rotation_interval</rdfs:label>
    <rdfs:comment>The interval between two consecutive rotations. Default rotation interval is 2 minutes</rdfs:comment>
    <rdfs:domain rdf:resource="http://example.org/onto/class/google_container_cluster"/>
    <rdfs:range rdf:resource="http://www.w3.org/2001/XMLSchema#string"/>
  </owl:DatatypeProperty>
  <owl:DatatypeProperty rdf:about="http://example.org/onto/prop/google_container_cluster_mode">
    <rdfs:label>mode</rdfs:label>
    <rdfs:comment>Sets the mode of the Kubernetes security posture API's off-cluster features. Available options include DISABLED, BASIC, and ENTERPRISE.</rdfs:comment>
    <rdfs:domain rdf:resource="http://example.org/onto/class/google_container_cluster"/>
    <rdfs:range rdf:resource="http://www.w3.org/2001/XMLSchema#string"/>
  </owl:DatatypeProperty>
  <owl:DatatypeProperty rdf:about="http://example.org/onto/prop/google_container_cluster_vulnerability_mode">
    <rdfs:label>vulnerability_mode</rdfs:label>
    <rdfs:comment>Sets the mode of the Kubernetes security posture API's workload vulnerability scanning. Available options include VULNERABILITY_DISABLED, VULNERABILITY_BASIC and VULNERABILITY_ENTERPRISE.</rdfs:comment>
    <rdfs:domain rdf:resource="http://example.org/onto/class/google_container_cluster"/>
    <rdfs:range rdf:resource="http://www.w3.org/2001/XMLSchema#string"/>
  </owl:DatatypeProperty>
  <owl:DatatypeProperty rdf:about="http://example.org/onto/prop/google_container_cluster_enabled">
    <rdfs:label>enabled</rdfs:label>
    <rdfs:comment>When enabled, services with external ips specified will be allowed.</rdfs:comment>
    <rdfs:domain rdf:resource="http://example.org/onto/class/google_container_cluster"/>
    <rdfs:range rdf:resource="http://www.w3.org/2001/XMLSchema#string"/>
  </owl:DatatypeProperty>
  <owl:DatatypeProperty rdf:about="http://example.org/onto/prop/google_container_cluster_create">
    <rdfs:label>create</rdfs:label>
    <rdfs:domain rdf:resource="http://example.org/onto/class/google_container_cluster"/>
    <rdfs:range rdf:resource="http://www.w3.org/2001/XMLSchema#string"/>
  </owl:DatatypeProperty>
  <owl:DatatypeProperty rdf:about="http://example.org/onto/prop/google_container_cluster_delete">
    <rdfs:label>delete</rdfs:label>
    <rdfs:domain rdf:resource="http://example.org/onto/class/google_container_cluster"/>
    <rdfs:range rdf:resource="http://www.w3.org/2001/XMLSchema#string"/>
  </owl:DatatypeProperty>
  <owl:DatatypeProperty rdf:about="http://example.org/onto/prop/google_container_cluster_read">
    <rdfs:label>read</rdfs:label>
    <rdfs:domain rdf:resource="http://example.org/onto/class/google_container_cluster"/>
    <rdfs:range rdf:resource="http://www.w3.org/2001/XMLSchema#string"/>
  </owl:DatatypeProperty>
  <owl:DatatypeProperty rdf:about="http://example.org/onto/prop/google_container_cluster_update">
    <rdfs:label>update</rdfs:label>
    <rdfs:domain rdf:resource="http://example.org/onto/class/google_container_cluster"/>
    <rdfs:range rdf:resource="http://www.w3.org/2001/XMLSchema#string"/>
  </owl:DatatypeProperty>
  <owl:DatatypeProperty rdf:about="http://example.org/onto/prop/google_container_cluster_aggregation_ca">
    <rdfs:label>aggregation_ca</rdfs:label>
    <rdfs:comment>The Certificate Authority Service caPool to use for the aggreation CA in this cluster.</rdfs:comment>
    <rdfs:domain rdf:resource="http://example.org/onto/class/google_container_cluster"/>
    <rdfs:range rdf:resource="http://www.w3.org/2001/XMLSchema#string"/>
  </owl:DatatypeProperty>
  <owl:DatatypeProperty rdf:about="http://example.org/onto/prop/google_container_cluster_cluster_ca">
    <rdfs:label>cluster_ca</rdfs:label>
    <rdfs:comment>The Certificate Authority Service caPool to use for the cluster CA in this cluster.</rdfs:comment>
    <rdfs:domain rdf:resource="http://example.org/onto/class/google_container_cluster"/>
    <rdfs:range rdf:resource="http://www.w3.org/2001/XMLSchema#string"/>
  </owl:DatatypeProperty>
  <owl:DatatypeProperty rdf:about="http://example.org/onto/prop/google_container_cluster_control_plane_disk_encryption_key">
    <rdfs:label>control_plane_disk_encryption_key</rdfs:label>
    <rdfs:comment>The Cloud KMS cryptoKey to use for Confidential Hyperdisk on the control plane nodes.</rdfs:comment>
    <rdfs:domain rdf:resource="http://example.org/onto/class/google_container_cluster"/>
    <rdfs:range rdf:resource="http://www.w3.org/2001/XMLSchema#string"/>
  </owl:DatatypeProperty>
  <owl:DatatypeProperty rdf:about="http://example.org/onto/prop/google_container_cluster_etcd_api_ca">
    <rdfs:label>etcd_api_ca</rdfs:label>
    <rdfs:comment>The Certificate Authority Service caPool to use for the etcd API CA in this cluster.</rdfs:comment>
    <rdfs:domain rdf:resource="http://example.org/onto/class/google_container_cluster"/>
    <rdfs:range rdf:resource="http://www.w3.org/2001/XMLSchema#string"/>
  </owl:DatatypeProperty>
  <owl:DatatypeProperty rdf:about="http://example.org/onto/prop/google_container_cluster_etcd_peer_ca">
    <rdfs:label>etcd_peer_ca</rdfs:label>
    <rdfs:comment>The Certificate Authority Service caPool to use for the etcd peer CA in this cluster.</rdfs:comment>
    <rdfs:domain rdf:resource="http://example.org/onto/class/google_container_cluster"/>
    <rdfs:range rdf:resource="http://www.w3.org/2001/XMLSchema#string"/>
  </owl:DatatypeProperty>
  <owl:DatatypeProperty rdf:about="http://example.org/onto/prop/google_container_cluster_gkeops_etcd_backup_encryption_key">
    <rdfs:label>gkeops_etcd_backup_encryption_key</rdfs:label>
    <rdfs:comment>Resource path of the Cloud KMS cryptoKey to use for encryption of internal etcd backups.</rdfs:comment>
    <rdfs:domain rdf:resource="http://example.org/onto/class/google_container_cluster"/>
    <rdfs:range rdf:resource="http://www.w3.org/2001/XMLSchema#string"/>
  </owl:DatatypeProperty>
  <owl:DatatypeProperty rdf:about="http://example.org/onto/prop/google_container_cluster_service_account_signing_keys">
    <rdfs:label>service_account_signing_keys</rdfs:label>
    <rdfs:comment>The Cloud KMS cryptoKeyVersions to use for signing service account JWTs issued by this cluster.</rdfs:comment>
    <rdfs:domain rdf:resource="http://example.org/onto/class/google_container_cluster"/>
    <rdfs:range rdf:resource="http://www.w3.org/2001/XMLSchema#string"/>
  </owl:DatatypeProperty>
  <owl:DatatypeProperty rdf:about="http://example.org/onto/prop/google_container_cluster_service_account_verification_keys">
    <rdfs:label>service_account_verification_keys</rdfs:label>
    <rdfs:comment>The Cloud KMS cryptoKeyVersions to use for verifying service account JWTs issued by this cluster.</rdfs:comment>
    <rdfs:domain rdf:resource="http://example.org/onto/class/google_container_cluster"/>
    <rdfs:range rdf:resource="http://www.w3.org/2001/XMLSchema#string"/>
  </owl:DatatypeProperty>
  <owl:DatatypeProperty rdf:about="http://example.org/onto/prop/google_container_cluster_enabled">
    <rdfs:label>enabled</rdfs:label>
    <rdfs:comment>Enables vertical pod autoscaling.</rdfs:comment>
    <rdfs:domain rdf:resource="http://example.org/onto/class/google_container_cluster"/>
    <rdfs:range rdf:resource="http://www.w3.org/2001/XMLSchema#string"/>
  </owl:DatatypeProperty>
  <owl:DatatypeProperty rdf:about="http://example.org/onto/prop/google_container_cluster_workload_pool">
    <rdfs:label>workload_pool</rdfs:label>
    <rdfs:comment>The workload pool to attach all Kubernetes service accounts to.</rdfs:comment>
    <rdfs:domain rdf:resource="http://example.org/onto/class/google_container_cluster"/>
    <rdfs:range rdf:resource="http://www.w3.org/2001/XMLSchema#string"/>
  </owl:DatatypeProperty>
</rdf:RDF>
