<?xml version="1.0" encoding="UTF-8"?>
<rdf:RDF
  xmlns:rdf="http://www.w3.org/1999/02/22-rdf-syntax-ns#"
  xmlns:rdfs="http://www.w3.org/2000/01/rdf-schema#"
  xmlns:owl="http://www.w3.org/2002/07/owl#"
  xmlns:xsd="http://www.w3.org/2001/XMLSchema#"
  xml:base="http://example.org/onto/">
  <owl:Class rdf:about="http://example.org/onto/class/google_bigquery_connection">
    <rdfs:label>google_bigquery_connection</rdfs:label>
    <rdfs:comment>#
#     ***     AUTO GENERATED CODE    ***    Type: MMv1     ***
#
# ----------------------------------------------------------------------------
#
#     This code is generated by Magic Modules using the following:
#
#     Configuration: https:#github.com/GoogleCloudPlatform/magic-modules/tree/main/mmv1/products/bigqueryconnection/Connection.yaml
#     Template:      https:#github.com/GoogleCloudPlatform/magic-modules/tree/main/mmv1/templates/terraform/resource.html.markdown.tmpl
#
#     DO NOT EDIT this file directly. Any changes made to this file will be
#     overwritten during the next generation cycle.
#
# ----------------------------------------------------------------------------
subcategory: "BigQuery Connection"
description: |-
  A connection allows BigQuery connections to external data sources.
---</rdfs:comment>
  </owl:Class>
  <owl:DatatypeProperty rdf:about="http://example.org/onto/prop/google_bigquery_connection_connection_id">
    <rdfs:label>connection_id</rdfs:label>
    <rdfs:comment>Optional connection id that should be assigned to the created connection.</rdfs:comment>
    <rdfs:domain rdf:resource="http://example.org/onto/class/google_bigquery_connection"/>
    <rdfs:range rdf:resource="http://www.w3.org/2001/XMLSchema#string"/>
  </owl:DatatypeProperty>
  <owl:DatatypeProperty rdf:about="http://example.org/onto/prop/google_bigquery_connection_description">
    <rdfs:label>description</rdfs:label>
    <rdfs:comment>A descriptive description for the connection</rdfs:comment>
    <rdfs:domain rdf:resource="http://example.org/onto/class/google_bigquery_connection"/>
    <rdfs:range rdf:resource="http://www.w3.org/2001/XMLSchema#string"/>
  </owl:DatatypeProperty>
  <owl:DatatypeProperty rdf:about="http://example.org/onto/prop/google_bigquery_connection_friendly_name">
    <rdfs:label>friendly_name</rdfs:label>
    <rdfs:comment>A descriptive name for the connection</rdfs:comment>
    <rdfs:domain rdf:resource="http://example.org/onto/class/google_bigquery_connection"/>
    <rdfs:range rdf:resource="http://www.w3.org/2001/XMLSchema#string"/>
  </owl:DatatypeProperty>
  <owl:DatatypeProperty rdf:about="http://example.org/onto/prop/google_bigquery_connection_has_credential">
    <rdfs:label>has_credential</rdfs:label>
    <rdfs:comment>True if the connection has credential assigned.</rdfs:comment>
    <rdfs:domain rdf:resource="http://example.org/onto/class/google_bigquery_connection"/>
    <rdfs:range rdf:resource="http://www.w3.org/2001/XMLSchema#string"/>
  </owl:DatatypeProperty>
  <owl:DatatypeProperty rdf:about="http://example.org/onto/prop/google_bigquery_connection_id">
    <rdfs:label>id</rdfs:label>
    <rdfs:domain rdf:resource="http://example.org/onto/class/google_bigquery_connection"/>
    <rdfs:range rdf:resource="http://www.w3.org/2001/XMLSchema#string"/>
  </owl:DatatypeProperty>
  <owl:DatatypeProperty rdf:about="http://example.org/onto/prop/google_bigquery_connection_kms_key_name">
    <rdfs:label>kms_key_name</rdfs:label>
    <rdfs:comment>Optional. The Cloud KMS key that is used for encryption.

Example: projects/[kms_project_id]/locations/[region]/keyRings/[key_region]/cryptoKeys/[key]</rdfs:comment>
    <rdfs:domain rdf:resource="http://example.org/onto/class/google_bigquery_connection"/>
    <rdfs:range rdf:resource="http://www.w3.org/2001/XMLSchema#string"/>
  </owl:DatatypeProperty>
  <owl:DatatypeProperty rdf:about="http://example.org/onto/prop/google_bigquery_connection_location">
    <rdfs:label>location</rdfs:label>
    <rdfs:comment>The geographic location where the connection should reside.
Cloud SQL instance must be in the same location as the connection
with following exceptions: Cloud SQL us-central1 maps to BigQuery US, Cloud SQL europe-west1 maps to BigQuery EU.
Examples: US, EU, asia-northeast1, us-central1, europe-west1.
Spanner Connections same as spanner region
AWS allowed regions are aws-us-east-1
Azure allowed regions are azure-eastus2</rdfs:comment>
    <rdfs:domain rdf:resource="http://example.org/onto/class/google_bigquery_connection"/>
    <rdfs:range rdf:resource="http://www.w3.org/2001/XMLSchema#string"/>
  </owl:DatatypeProperty>
  <owl:DatatypeProperty rdf:about="http://example.org/onto/prop/google_bigquery_connection_name">
    <rdfs:label>name</rdfs:label>
    <rdfs:comment>The resource name of the connection in the form of:
"projects/{project_id}/locations/{location_id}/connections/{connectionId}"</rdfs:comment>
    <rdfs:domain rdf:resource="http://example.org/onto/class/google_bigquery_connection"/>
    <rdfs:range rdf:resource="http://www.w3.org/2001/XMLSchema#string"/>
  </owl:DatatypeProperty>
  <owl:DatatypeProperty rdf:about="http://example.org/onto/prop/google_bigquery_connection_project">
    <rdfs:label>project</rdfs:label>
    <rdfs:domain rdf:resource="http://example.org/onto/class/google_bigquery_connection"/>
    <rdfs:range rdf:resource="http://www.w3.org/2001/XMLSchema#string"/>
  </owl:DatatypeProperty>
  <owl:DatatypeProperty rdf:about="http://example.org/onto/prop/google_bigquery_connection_iam_role_id">
    <rdfs:label>iam_role_id</rdfs:label>
    <rdfs:comment>The userâ€™s AWS IAM Role that trusts the Google-owned AWS IAM user Connection.</rdfs:comment>
    <rdfs:domain rdf:resource="http://example.org/onto/class/google_bigquery_connection"/>
    <rdfs:range rdf:resource="http://www.w3.org/2001/XMLSchema#string"/>
  </owl:DatatypeProperty>
  <owl:DatatypeProperty rdf:about="http://example.org/onto/prop/google_bigquery_connection_identity">
    <rdfs:label>identity</rdfs:label>
    <rdfs:comment>A unique Google-owned and Google-generated identity for the Connection. This identity will be used to access the user's AWS IAM Role.</rdfs:comment>
    <rdfs:domain rdf:resource="http://example.org/onto/class/google_bigquery_connection"/>
    <rdfs:range rdf:resource="http://www.w3.org/2001/XMLSchema#string"/>
  </owl:DatatypeProperty>
  <owl:DatatypeProperty rdf:about="http://example.org/onto/prop/google_bigquery_connection_application">
    <rdfs:label>application</rdfs:label>
    <rdfs:comment>The name of the Azure Active Directory Application.</rdfs:comment>
    <rdfs:domain rdf:resource="http://example.org/onto/class/google_bigquery_connection"/>
    <rdfs:range rdf:resource="http://www.w3.org/2001/XMLSchema#string"/>
  </owl:DatatypeProperty>
  <owl:DatatypeProperty rdf:about="http://example.org/onto/prop/google_bigquery_connection_client_id">
    <rdfs:label>client_id</rdfs:label>
    <rdfs:comment>The client id of the Azure Active Directory Application.</rdfs:comment>
    <rdfs:domain rdf:resource="http://example.org/onto/class/google_bigquery_connection"/>
    <rdfs:range rdf:resource="http://www.w3.org/2001/XMLSchema#string"/>
  </owl:DatatypeProperty>
  <owl:DatatypeProperty rdf:about="http://example.org/onto/prop/google_bigquery_connection_customer_tenant_id">
    <rdfs:label>customer_tenant_id</rdfs:label>
    <rdfs:comment>The id of customer's directory that host the data.</rdfs:comment>
    <rdfs:domain rdf:resource="http://example.org/onto/class/google_bigquery_connection"/>
    <rdfs:range rdf:resource="http://www.w3.org/2001/XMLSchema#string"/>
  </owl:DatatypeProperty>
  <owl:DatatypeProperty rdf:about="http://example.org/onto/prop/google_bigquery_connection_federated_application_client_id">
    <rdfs:label>federated_application_client_id</rdfs:label>
    <rdfs:comment>The Azure Application (client) ID where the federated credentials will be hosted.</rdfs:comment>
    <rdfs:domain rdf:resource="http://example.org/onto/class/google_bigquery_connection"/>
    <rdfs:range rdf:resource="http://www.w3.org/2001/XMLSchema#string"/>
  </owl:DatatypeProperty>
  <owl:DatatypeProperty rdf:about="http://example.org/onto/prop/google_bigquery_connection_identity">
    <rdfs:label>identity</rdfs:label>
    <rdfs:comment>A unique Google-owned and Google-generated identity for the Connection. This identity will be used to access the user's Azure Active Directory Application.</rdfs:comment>
    <rdfs:domain rdf:resource="http://example.org/onto/class/google_bigquery_connection"/>
    <rdfs:range rdf:resource="http://www.w3.org/2001/XMLSchema#string"/>
  </owl:DatatypeProperty>
  <owl:DatatypeProperty rdf:about="http://example.org/onto/prop/google_bigquery_connection_object_id">
    <rdfs:label>object_id</rdfs:label>
    <rdfs:comment>The object id of the Azure Active Directory Application.</rdfs:comment>
    <rdfs:domain rdf:resource="http://example.org/onto/class/google_bigquery_connection"/>
    <rdfs:range rdf:resource="http://www.w3.org/2001/XMLSchema#string"/>
  </owl:DatatypeProperty>
  <owl:DatatypeProperty rdf:about="http://example.org/onto/prop/google_bigquery_connection_redirect_uri">
    <rdfs:label>redirect_uri</rdfs:label>
    <rdfs:comment>The URL user will be redirected to after granting consent during connection setup.</rdfs:comment>
    <rdfs:domain rdf:resource="http://example.org/onto/class/google_bigquery_connection"/>
    <rdfs:range rdf:resource="http://www.w3.org/2001/XMLSchema#string"/>
  </owl:DatatypeProperty>
  <owl:DatatypeProperty rdf:about="http://example.org/onto/prop/google_bigquery_connection_service_account_id">
    <rdfs:label>service_account_id</rdfs:label>
    <rdfs:comment>The account ID of the service created for the purpose of this connection.</rdfs:comment>
    <rdfs:domain rdf:resource="http://example.org/onto/class/google_bigquery_connection"/>
    <rdfs:range rdf:resource="http://www.w3.org/2001/XMLSchema#string"/>
  </owl:DatatypeProperty>
  <owl:DatatypeProperty rdf:about="http://example.org/onto/prop/google_bigquery_connection_database">
    <rdfs:label>database</rdfs:label>
    <rdfs:comment>Cloud Spanner database in the form 'project/instance/database'.</rdfs:comment>
    <rdfs:domain rdf:resource="http://example.org/onto/class/google_bigquery_connection"/>
    <rdfs:range rdf:resource="http://www.w3.org/2001/XMLSchema#string"/>
  </owl:DatatypeProperty>
  <owl:DatatypeProperty rdf:about="http://example.org/onto/prop/google_bigquery_connection_database_role">
    <rdfs:label>database_role</rdfs:label>
    <rdfs:comment>Cloud Spanner database role for fine-grained access control. The Cloud Spanner admin should have provisioned the database role with appropriate permissions, such as 'SELECT' and 'INSERT'. Other users should only use roles provided by their Cloud Spanner admins. The database role name must start with a letter, and can only contain letters, numbers, and underscores. For more details, see https://cloud.google.com/spanner/docs/fgac-about.</rdfs:comment>
    <rdfs:domain rdf:resource="http://example.org/onto/class/google_bigquery_connection"/>
    <rdfs:range rdf:resource="http://www.w3.org/2001/XMLSchema#string"/>
  </owl:DatatypeProperty>
  <owl:DatatypeProperty rdf:about="http://example.org/onto/prop/google_bigquery_connection_max_parallelism">
    <rdfs:label>max_parallelism</rdfs:label>
    <rdfs:comment>Allows setting max parallelism per query when executing on Spanner independent compute resources. If unspecified, default values of parallelism are chosen that are dependent on the Cloud Spanner instance configuration. 'useParallelism' and 'useDataBoost' must be set when setting max parallelism.</rdfs:comment>
    <rdfs:domain rdf:resource="http://example.org/onto/class/google_bigquery_connection"/>
    <rdfs:range rdf:resource="http://www.w3.org/2001/XMLSchema#string"/>
  </owl:DatatypeProperty>
  <owl:DatatypeProperty rdf:about="http://example.org/onto/prop/google_bigquery_connection_use_data_boost">
    <rdfs:label>use_data_boost</rdfs:label>
    <rdfs:comment>If set, the request will be executed via Spanner independent compute resources. 'use_parallelism' must be set when using data boost.</rdfs:comment>
    <rdfs:domain rdf:resource="http://example.org/onto/class/google_bigquery_connection"/>
    <rdfs:range rdf:resource="http://www.w3.org/2001/XMLSchema#string"/>
  </owl:DatatypeProperty>
  <owl:DatatypeProperty rdf:about="http://example.org/onto/prop/google_bigquery_connection_use_parallelism">
    <rdfs:label>use_parallelism</rdfs:label>
    <rdfs:comment>If parallelism should be used when reading from Cloud Spanner.</rdfs:comment>
    <rdfs:domain rdf:resource="http://example.org/onto/class/google_bigquery_connection"/>
    <rdfs:range rdf:resource="http://www.w3.org/2001/XMLSchema#string"/>
  </owl:DatatypeProperty>
  <owl:DatatypeProperty rdf:about="http://example.org/onto/prop/google_bigquery_connection_use_serverless_analytics">
    <rdfs:label>use_serverless_analytics</rdfs:label>
    <rdfs:comment>If the serverless analytics service should be used to read data from Cloud Spanner. 'useParallelism' must be set when using serverless analytics.</rdfs:comment>
    <rdfs:domain rdf:resource="http://example.org/onto/class/google_bigquery_connection"/>
    <rdfs:range rdf:resource="http://www.w3.org/2001/XMLSchema#string"/>
  </owl:DatatypeProperty>
  <owl:DatatypeProperty rdf:about="http://example.org/onto/prop/google_bigquery_connection_database">
    <rdfs:label>database</rdfs:label>
    <rdfs:comment>Database name.</rdfs:comment>
    <rdfs:domain rdf:resource="http://example.org/onto/class/google_bigquery_connection"/>
    <rdfs:range rdf:resource="http://www.w3.org/2001/XMLSchema#string"/>
  </owl:DatatypeProperty>
  <owl:DatatypeProperty rdf:about="http://example.org/onto/prop/google_bigquery_connection_instance_id">
    <rdfs:label>instance_id</rdfs:label>
    <rdfs:comment>Cloud SQL instance ID in the form project:location:instance.</rdfs:comment>
    <rdfs:domain rdf:resource="http://example.org/onto/class/google_bigquery_connection"/>
    <rdfs:range rdf:resource="http://www.w3.org/2001/XMLSchema#string"/>
  </owl:DatatypeProperty>
  <owl:DatatypeProperty rdf:about="http://example.org/onto/prop/google_bigquery_connection_service_account_id">
    <rdfs:label>service_account_id</rdfs:label>
    <rdfs:comment>When the connection is used in the context of an operation in BigQuery, this service account will serve as the identity being used for connecting to the CloudSQL instance specified in this connection.</rdfs:comment>
    <rdfs:domain rdf:resource="http://example.org/onto/class/google_bigquery_connection"/>
    <rdfs:range rdf:resource="http://www.w3.org/2001/XMLSchema#string"/>
  </owl:DatatypeProperty>
  <owl:DatatypeProperty rdf:about="http://example.org/onto/prop/google_bigquery_connection_type">
    <rdfs:label>type</rdfs:label>
    <rdfs:comment>Type of the Cloud SQL database. Possible values: ["DATABASE_TYPE_UNSPECIFIED", "POSTGRES", "MYSQL"]</rdfs:comment>
    <rdfs:domain rdf:resource="http://example.org/onto/class/google_bigquery_connection"/>
    <rdfs:range rdf:resource="http://www.w3.org/2001/XMLSchema#string"/>
  </owl:DatatypeProperty>
  <owl:DatatypeProperty rdf:about="http://example.org/onto/prop/google_bigquery_connection_password">
    <rdfs:label>password</rdfs:label>
    <rdfs:comment>Password for database.</rdfs:comment>
    <rdfs:domain rdf:resource="http://example.org/onto/class/google_bigquery_connection"/>
    <rdfs:range rdf:resource="http://www.w3.org/2001/XMLSchema#string"/>
  </owl:DatatypeProperty>
  <owl:DatatypeProperty rdf:about="http://example.org/onto/prop/google_bigquery_connection_username">
    <rdfs:label>username</rdfs:label>
    <rdfs:comment>Username for database.</rdfs:comment>
    <rdfs:domain rdf:resource="http://example.org/onto/class/google_bigquery_connection"/>
    <rdfs:range rdf:resource="http://www.w3.org/2001/XMLSchema#string"/>
  </owl:DatatypeProperty>
  <owl:DatatypeProperty rdf:about="http://example.org/onto/prop/google_bigquery_connection_service_account_id">
    <rdfs:label>service_account_id</rdfs:label>
    <rdfs:comment>The account ID of the service created for the purpose of this connection.</rdfs:comment>
    <rdfs:domain rdf:resource="http://example.org/onto/class/google_bigquery_connection"/>
    <rdfs:range rdf:resource="http://www.w3.org/2001/XMLSchema#string"/>
  </owl:DatatypeProperty>
  <owl:DatatypeProperty rdf:about="http://example.org/onto/prop/google_bigquery_connection_metastore_service">
    <rdfs:label>metastore_service</rdfs:label>
    <rdfs:comment>Resource name of an existing Dataproc Metastore service in the form of projects/[projectId]/locations/[region]/services/[serviceId].</rdfs:comment>
    <rdfs:domain rdf:resource="http://example.org/onto/class/google_bigquery_connection"/>
    <rdfs:range rdf:resource="http://www.w3.org/2001/XMLSchema#string"/>
  </owl:DatatypeProperty>
  <owl:DatatypeProperty rdf:about="http://example.org/onto/prop/google_bigquery_connection_dataproc_cluster">
    <rdfs:label>dataproc_cluster</rdfs:label>
    <rdfs:comment>Resource name of an existing Dataproc Cluster to act as a Spark History Server for the connection if the form of projects/[projectId]/regions/[region]/clusters/[cluster_name].</rdfs:comment>
    <rdfs:domain rdf:resource="http://example.org/onto/class/google_bigquery_connection"/>
    <rdfs:range rdf:resource="http://www.w3.org/2001/XMLSchema#string"/>
  </owl:DatatypeProperty>
  <owl:DatatypeProperty rdf:about="http://example.org/onto/prop/google_bigquery_connection_create">
    <rdfs:label>create</rdfs:label>
    <rdfs:domain rdf:resource="http://example.org/onto/class/google_bigquery_connection"/>
    <rdfs:range rdf:resource="http://www.w3.org/2001/XMLSchema#string"/>
  </owl:DatatypeProperty>
  <owl:DatatypeProperty rdf:about="http://example.org/onto/prop/google_bigquery_connection_delete">
    <rdfs:label>delete</rdfs:label>
    <rdfs:domain rdf:resource="http://example.org/onto/class/google_bigquery_connection"/>
    <rdfs:range rdf:resource="http://www.w3.org/2001/XMLSchema#string"/>
  </owl:DatatypeProperty>
  <owl:DatatypeProperty rdf:about="http://example.org/onto/prop/google_bigquery_connection_update">
    <rdfs:label>update</rdfs:label>
    <rdfs:domain rdf:resource="http://example.org/onto/class/google_bigquery_connection"/>
    <rdfs:range rdf:resource="http://www.w3.org/2001/XMLSchema#string"/>
  </owl:DatatypeProperty>
</rdf:RDF>
