<?xml version="1.0" encoding="UTF-8"?>
<rdf:RDF
  xmlns:rdf="http://www.w3.org/1999/02/22-rdf-syntax-ns#"
  xmlns:rdfs="http://www.w3.org/2000/01/rdf-schema#"
  xmlns:owl="http://www.w3.org/2002/07/owl#"
  xmlns:xsd="http://www.w3.org/2001/XMLSchema#"
  xml:base="http://example.org/onto/">
  <owl:Class rdf:about="http://example.org/onto/class/google_network_connectivity_policy_based_route">
    <rdfs:label>google_network_connectivity_policy_based_route</rdfs:label>
    <rdfs:comment>#
#     ***     AUTO GENERATED CODE    ***    Type: MMv1     ***
#
# ----------------------------------------------------------------------------
#
#     This code is generated by Magic Modules using the following:
#
#     Configuration: https:#github.com/GoogleCloudPlatform/magic-modules/tree/main/mmv1/products/networkconnectivity/PolicyBasedRoute.yaml
#     Template:      https:#github.com/GoogleCloudPlatform/magic-modules/tree/main/mmv1/templates/terraform/resource.html.markdown.tmpl
#
#     DO NOT EDIT this file directly. Any changes made to this file will be
#     overwritten during the next generation cycle.
#
# ----------------------------------------------------------------------------
subcategory: "Network Connectivity"
description: |-
  Policy-based Routes are more powerful routes that route L4 network traffic based on not just destination IP, but also source IP, protocol and more.
---</rdfs:comment>
  </owl:Class>
  <owl:DatatypeProperty rdf:about="http://example.org/onto/prop/google_network_connectivity_policy_based_route_create_time">
    <rdfs:label>create_time</rdfs:label>
    <rdfs:comment>Time when the policy-based route was created.</rdfs:comment>
    <rdfs:domain rdf:resource="http://example.org/onto/class/google_network_connectivity_policy_based_route"/>
    <rdfs:range rdf:resource="http://www.w3.org/2001/XMLSchema#string"/>
  </owl:DatatypeProperty>
  <owl:DatatypeProperty rdf:about="http://example.org/onto/prop/google_network_connectivity_policy_based_route_description">
    <rdfs:label>description</rdfs:label>
    <rdfs:comment>An optional description of this resource.</rdfs:comment>
    <rdfs:domain rdf:resource="http://example.org/onto/class/google_network_connectivity_policy_based_route"/>
    <rdfs:range rdf:resource="http://www.w3.org/2001/XMLSchema#string"/>
  </owl:DatatypeProperty>
  <owl:DatatypeProperty rdf:about="http://example.org/onto/prop/google_network_connectivity_policy_based_route_effective_labels">
    <rdfs:label>effective_labels</rdfs:label>
    <rdfs:comment>All of labels (key/value pairs) present on the resource in GCP, including the labels configured through Terraform, other clients and services.</rdfs:comment>
    <rdfs:domain rdf:resource="http://example.org/onto/class/google_network_connectivity_policy_based_route"/>
    <rdfs:range rdf:resource="http://www.w3.org/2001/XMLSchema#string"/>
  </owl:DatatypeProperty>
  <owl:DatatypeProperty rdf:about="http://example.org/onto/prop/google_network_connectivity_policy_based_route_id">
    <rdfs:label>id</rdfs:label>
    <rdfs:domain rdf:resource="http://example.org/onto/class/google_network_connectivity_policy_based_route"/>
    <rdfs:range rdf:resource="http://www.w3.org/2001/XMLSchema#string"/>
  </owl:DatatypeProperty>
  <owl:DatatypeProperty rdf:about="http://example.org/onto/prop/google_network_connectivity_policy_based_route_kind">
    <rdfs:label>kind</rdfs:label>
    <rdfs:comment>Type of this resource.</rdfs:comment>
    <rdfs:domain rdf:resource="http://example.org/onto/class/google_network_connectivity_policy_based_route"/>
    <rdfs:range rdf:resource="http://www.w3.org/2001/XMLSchema#string"/>
  </owl:DatatypeProperty>
  <owl:DatatypeProperty rdf:about="http://example.org/onto/prop/google_network_connectivity_policy_based_route_labels">
    <rdfs:label>labels</rdfs:label>
    <rdfs:comment>User-defined labels.


**Note**: This field is non-authoritative, and will only manage the labels present in your configuration.
Please refer to the field 'effective_labels' for all of the labels present on the resource.</rdfs:comment>
    <rdfs:domain rdf:resource="http://example.org/onto/class/google_network_connectivity_policy_based_route"/>
    <rdfs:range rdf:resource="http://www.w3.org/2001/XMLSchema#string"/>
  </owl:DatatypeProperty>
  <owl:DatatypeProperty rdf:about="http://example.org/onto/prop/google_network_connectivity_policy_based_route_name">
    <rdfs:label>name</rdfs:label>
    <rdfs:comment>The name of the policy based route.</rdfs:comment>
    <rdfs:domain rdf:resource="http://example.org/onto/class/google_network_connectivity_policy_based_route"/>
    <rdfs:range rdf:resource="http://www.w3.org/2001/XMLSchema#string"/>
  </owl:DatatypeProperty>
  <owl:DatatypeProperty rdf:about="http://example.org/onto/prop/google_network_connectivity_policy_based_route_network">
    <rdfs:label>network</rdfs:label>
    <rdfs:comment>Fully-qualified URL of the network that this route applies to, for example: projects/my-project/global/networks/my-network.</rdfs:comment>
    <rdfs:domain rdf:resource="http://example.org/onto/class/google_network_connectivity_policy_based_route"/>
    <rdfs:range rdf:resource="http://www.w3.org/2001/XMLSchema#string"/>
  </owl:DatatypeProperty>
  <owl:DatatypeProperty rdf:about="http://example.org/onto/prop/google_network_connectivity_policy_based_route_next_hop_ilb_ip">
    <rdfs:label>next_hop_ilb_ip</rdfs:label>
    <rdfs:comment>The IP address of a global-access-enabled L4 ILB that is the next hop for matching packets.</rdfs:comment>
    <rdfs:domain rdf:resource="http://example.org/onto/class/google_network_connectivity_policy_based_route"/>
    <rdfs:range rdf:resource="http://www.w3.org/2001/XMLSchema#string"/>
  </owl:DatatypeProperty>
  <owl:DatatypeProperty rdf:about="http://example.org/onto/prop/google_network_connectivity_policy_based_route_next_hop_other_routes">
    <rdfs:label>next_hop_other_routes</rdfs:label>
    <rdfs:comment>Other routes that will be referenced to determine the next hop of the packet. Possible values: ["DEFAULT_ROUTING"]</rdfs:comment>
    <rdfs:domain rdf:resource="http://example.org/onto/class/google_network_connectivity_policy_based_route"/>
    <rdfs:range rdf:resource="http://www.w3.org/2001/XMLSchema#string"/>
  </owl:DatatypeProperty>
  <owl:DatatypeProperty rdf:about="http://example.org/onto/prop/google_network_connectivity_policy_based_route_priority">
    <rdfs:label>priority</rdfs:label>
    <rdfs:comment>The priority of this policy-based route. Priority is used to break ties in cases where there are more than one matching policy-based routes found. In cases where multiple policy-based routes are matched, the one with the lowest-numbered priority value wins. The default value is 1000. The priority value must be from 1 to 65535, inclusive.</rdfs:comment>
    <rdfs:domain rdf:resource="http://example.org/onto/class/google_network_connectivity_policy_based_route"/>
    <rdfs:range rdf:resource="http://www.w3.org/2001/XMLSchema#string"/>
  </owl:DatatypeProperty>
  <owl:DatatypeProperty rdf:about="http://example.org/onto/prop/google_network_connectivity_policy_based_route_project">
    <rdfs:label>project</rdfs:label>
    <rdfs:domain rdf:resource="http://example.org/onto/class/google_network_connectivity_policy_based_route"/>
    <rdfs:range rdf:resource="http://www.w3.org/2001/XMLSchema#string"/>
  </owl:DatatypeProperty>
  <owl:DatatypeProperty rdf:about="http://example.org/onto/prop/google_network_connectivity_policy_based_route_terraform_labels">
    <rdfs:label>terraform_labels</rdfs:label>
    <rdfs:comment>The combination of labels configured directly on the resource
 and default labels configured on the provider.</rdfs:comment>
    <rdfs:domain rdf:resource="http://example.org/onto/class/google_network_connectivity_policy_based_route"/>
    <rdfs:range rdf:resource="http://www.w3.org/2001/XMLSchema#string"/>
  </owl:DatatypeProperty>
  <owl:DatatypeProperty rdf:about="http://example.org/onto/prop/google_network_connectivity_policy_based_route_update_time">
    <rdfs:label>update_time</rdfs:label>
    <rdfs:comment>Time when the policy-based route was created.</rdfs:comment>
    <rdfs:domain rdf:resource="http://example.org/onto/class/google_network_connectivity_policy_based_route"/>
    <rdfs:range rdf:resource="http://www.w3.org/2001/XMLSchema#string"/>
  </owl:DatatypeProperty>
  <owl:DatatypeProperty rdf:about="http://example.org/onto/prop/google_network_connectivity_policy_based_route_warnings">
    <rdfs:label>warnings</rdfs:label>
    <rdfs:comment>If potential misconfigurations are detected for this route, this field will be populated with warning messages.</rdfs:comment>
    <rdfs:domain rdf:resource="http://example.org/onto/class/google_network_connectivity_policy_based_route"/>
    <rdfs:range rdf:resource="http://www.w3.org/2001/XMLSchema#string"/>
  </owl:DatatypeProperty>
  <owl:DatatypeProperty rdf:about="http://example.org/onto/prop/google_network_connectivity_policy_based_route_dest_range">
    <rdfs:label>dest_range</rdfs:label>
    <rdfs:comment>The destination IP range of outgoing packets that this policy-based route applies to. Default is "0.0.0.0/0".</rdfs:comment>
    <rdfs:domain rdf:resource="http://example.org/onto/class/google_network_connectivity_policy_based_route"/>
    <rdfs:range rdf:resource="http://www.w3.org/2001/XMLSchema#string"/>
  </owl:DatatypeProperty>
  <owl:DatatypeProperty rdf:about="http://example.org/onto/prop/google_network_connectivity_policy_based_route_ip_protocol">
    <rdfs:label>ip_protocol</rdfs:label>
    <rdfs:comment>The IP protocol that this policy-based route applies to. Valid values are 'TCP', 'UDP', and 'ALL'. Default is 'ALL'.</rdfs:comment>
    <rdfs:domain rdf:resource="http://example.org/onto/class/google_network_connectivity_policy_based_route"/>
    <rdfs:range rdf:resource="http://www.w3.org/2001/XMLSchema#string"/>
  </owl:DatatypeProperty>
  <owl:DatatypeProperty rdf:about="http://example.org/onto/prop/google_network_connectivity_policy_based_route_protocol_version">
    <rdfs:label>protocol_version</rdfs:label>
    <rdfs:comment>Internet protocol versions this policy-based route applies to. Possible values: ["IPV4", "IPV6"]</rdfs:comment>
    <rdfs:domain rdf:resource="http://example.org/onto/class/google_network_connectivity_policy_based_route"/>
    <rdfs:range rdf:resource="http://www.w3.org/2001/XMLSchema#string"/>
  </owl:DatatypeProperty>
  <owl:DatatypeProperty rdf:about="http://example.org/onto/prop/google_network_connectivity_policy_based_route_src_range">
    <rdfs:label>src_range</rdfs:label>
    <rdfs:comment>The source IP range of outgoing packets that this policy-based route applies to. Default is "0.0.0.0/0".</rdfs:comment>
    <rdfs:domain rdf:resource="http://example.org/onto/class/google_network_connectivity_policy_based_route"/>
    <rdfs:range rdf:resource="http://www.w3.org/2001/XMLSchema#string"/>
  </owl:DatatypeProperty>
  <owl:DatatypeProperty rdf:about="http://example.org/onto/prop/google_network_connectivity_policy_based_route_region">
    <rdfs:label>region</rdfs:label>
    <rdfs:comment>Cloud region to install this policy-based route on for Interconnect attachments. Use 'all' to install it on all Interconnect attachments.</rdfs:comment>
    <rdfs:domain rdf:resource="http://example.org/onto/class/google_network_connectivity_policy_based_route"/>
    <rdfs:range rdf:resource="http://www.w3.org/2001/XMLSchema#string"/>
  </owl:DatatypeProperty>
  <owl:DatatypeProperty rdf:about="http://example.org/onto/prop/google_network_connectivity_policy_based_route_create">
    <rdfs:label>create</rdfs:label>
    <rdfs:domain rdf:resource="http://example.org/onto/class/google_network_connectivity_policy_based_route"/>
    <rdfs:range rdf:resource="http://www.w3.org/2001/XMLSchema#string"/>
  </owl:DatatypeProperty>
  <owl:DatatypeProperty rdf:about="http://example.org/onto/prop/google_network_connectivity_policy_based_route_delete">
    <rdfs:label>delete</rdfs:label>
    <rdfs:domain rdf:resource="http://example.org/onto/class/google_network_connectivity_policy_based_route"/>
    <rdfs:range rdf:resource="http://www.w3.org/2001/XMLSchema#string"/>
  </owl:DatatypeProperty>
  <owl:DatatypeProperty rdf:about="http://example.org/onto/prop/google_network_connectivity_policy_based_route_update">
    <rdfs:label>update</rdfs:label>
    <rdfs:domain rdf:resource="http://example.org/onto/class/google_network_connectivity_policy_based_route"/>
    <rdfs:range rdf:resource="http://www.w3.org/2001/XMLSchema#string"/>
  </owl:DatatypeProperty>
  <owl:DatatypeProperty rdf:about="http://example.org/onto/prop/google_network_connectivity_policy_based_route_tags">
    <rdfs:label>tags</rdfs:label>
    <rdfs:comment>A list of VM instance tags that this policy-based route applies to. VM instances that have ANY of tags specified here will install this PBR.</rdfs:comment>
    <rdfs:domain rdf:resource="http://example.org/onto/class/google_network_connectivity_policy_based_route"/>
    <rdfs:range rdf:resource="http://www.w3.org/2001/XMLSchema#string"/>
  </owl:DatatypeProperty>
</rdf:RDF>
