<?xml version="1.0" encoding="UTF-8"?>
<rdf:RDF
  xmlns:rdf="http://www.w3.org/1999/02/22-rdf-syntax-ns#"
  xmlns:rdfs="http://www.w3.org/2000/01/rdf-schema#"
  xmlns:owl="http://www.w3.org/2002/07/owl#"
  xmlns:xsd="http://www.w3.org/2001/XMLSchema#"
  xml:base="http://example.org/onto/">
  <owl:Class rdf:about="http://example.org/onto/class/google_network_services_wasm_plugin">
    <rdfs:label>google_network_services_wasm_plugin</rdfs:label>
    <rdfs:comment>#
#     ***     AUTO GENERATED CODE    ***    Type: MMv1     ***
#
# ----------------------------------------------------------------------------
#
#     This code is generated by Magic Modules using the following:
#
#     Configuration: https:#github.com/GoogleCloudPlatform/magic-modules/tree/main/mmv1/products/networkservices/WasmPlugin.yaml
#     Template:      https:#github.com/GoogleCloudPlatform/magic-modules/tree/main/mmv1/templates/terraform/resource.html.markdown.tmpl
#
#     DO NOT EDIT this file directly. Any changes made to this file will be
#     overwritten during the next generation cycle.
#
# ----------------------------------------------------------------------------
subcategory: "Network Services"
description: |-
  WasmPlugin is a resource representing a service executing a customer-provided Wasm module.
---</rdfs:comment>
  </owl:Class>
  <owl:DatatypeProperty rdf:about="http://example.org/onto/prop/google_network_services_wasm_plugin_create_time">
    <rdfs:label>create_time</rdfs:label>
    <rdfs:comment>Output only. The timestamp when the resource was created.</rdfs:comment>
    <rdfs:domain rdf:resource="http://example.org/onto/class/google_network_services_wasm_plugin"/>
    <rdfs:range rdf:resource="http://www.w3.org/2001/XMLSchema#string"/>
  </owl:DatatypeProperty>
  <owl:DatatypeProperty rdf:about="http://example.org/onto/prop/google_network_services_wasm_plugin_description">
    <rdfs:label>description</rdfs:label>
    <rdfs:comment>Optional. A human-readable description of the resource.</rdfs:comment>
    <rdfs:domain rdf:resource="http://example.org/onto/class/google_network_services_wasm_plugin"/>
    <rdfs:range rdf:resource="http://www.w3.org/2001/XMLSchema#string"/>
  </owl:DatatypeProperty>
  <owl:DatatypeProperty rdf:about="http://example.org/onto/prop/google_network_services_wasm_plugin_effective_labels">
    <rdfs:label>effective_labels</rdfs:label>
    <rdfs:comment>All of labels (key/value pairs) present on the resource in GCP, including the labels configured through Terraform, other clients and services.</rdfs:comment>
    <rdfs:domain rdf:resource="http://example.org/onto/class/google_network_services_wasm_plugin"/>
    <rdfs:range rdf:resource="http://www.w3.org/2001/XMLSchema#string"/>
  </owl:DatatypeProperty>
  <owl:DatatypeProperty rdf:about="http://example.org/onto/prop/google_network_services_wasm_plugin_id">
    <rdfs:label>id</rdfs:label>
    <rdfs:domain rdf:resource="http://example.org/onto/class/google_network_services_wasm_plugin"/>
    <rdfs:range rdf:resource="http://www.w3.org/2001/XMLSchema#string"/>
  </owl:DatatypeProperty>
  <owl:DatatypeProperty rdf:about="http://example.org/onto/prop/google_network_services_wasm_plugin_labels">
    <rdfs:label>labels</rdfs:label>
    <rdfs:comment>Optional. Set of labels associated with the WasmPlugin resource.

**Note**: This field is non-authoritative, and will only manage the labels present in your configuration.
Please refer to the field 'effective_labels' for all of the labels present on the resource.</rdfs:comment>
    <rdfs:domain rdf:resource="http://example.org/onto/class/google_network_services_wasm_plugin"/>
    <rdfs:range rdf:resource="http://www.w3.org/2001/XMLSchema#string"/>
  </owl:DatatypeProperty>
  <owl:DatatypeProperty rdf:about="http://example.org/onto/prop/google_network_services_wasm_plugin_location">
    <rdfs:label>location</rdfs:label>
    <rdfs:comment>The location of the traffic extension</rdfs:comment>
    <rdfs:domain rdf:resource="http://example.org/onto/class/google_network_services_wasm_plugin"/>
    <rdfs:range rdf:resource="http://www.w3.org/2001/XMLSchema#string"/>
  </owl:DatatypeProperty>
  <owl:DatatypeProperty rdf:about="http://example.org/onto/prop/google_network_services_wasm_plugin_main_version_id">
    <rdfs:label>main_version_id</rdfs:label>
    <rdfs:comment>The ID of the WasmPluginVersion resource that is the currently serving one. The version referred to must be a child of this WasmPlugin resource and should be listed in the "versions" field.</rdfs:comment>
    <rdfs:domain rdf:resource="http://example.org/onto/class/google_network_services_wasm_plugin"/>
    <rdfs:range rdf:resource="http://www.w3.org/2001/XMLSchema#string"/>
  </owl:DatatypeProperty>
  <owl:DatatypeProperty rdf:about="http://example.org/onto/prop/google_network_services_wasm_plugin_name">
    <rdfs:label>name</rdfs:label>
    <rdfs:comment>Identifier. Name of the WasmPlugin resource.</rdfs:comment>
    <rdfs:domain rdf:resource="http://example.org/onto/class/google_network_services_wasm_plugin"/>
    <rdfs:range rdf:resource="http://www.w3.org/2001/XMLSchema#string"/>
  </owl:DatatypeProperty>
  <owl:DatatypeProperty rdf:about="http://example.org/onto/prop/google_network_services_wasm_plugin_project">
    <rdfs:label>project</rdfs:label>
    <rdfs:domain rdf:resource="http://example.org/onto/class/google_network_services_wasm_plugin"/>
    <rdfs:range rdf:resource="http://www.w3.org/2001/XMLSchema#string"/>
  </owl:DatatypeProperty>
  <owl:DatatypeProperty rdf:about="http://example.org/onto/prop/google_network_services_wasm_plugin_terraform_labels">
    <rdfs:label>terraform_labels</rdfs:label>
    <rdfs:comment>The combination of labels configured directly on the resource
 and default labels configured on the provider.</rdfs:comment>
    <rdfs:domain rdf:resource="http://example.org/onto/class/google_network_services_wasm_plugin"/>
    <rdfs:range rdf:resource="http://www.w3.org/2001/XMLSchema#string"/>
  </owl:DatatypeProperty>
  <owl:DatatypeProperty rdf:about="http://example.org/onto/prop/google_network_services_wasm_plugin_update_time">
    <rdfs:label>update_time</rdfs:label>
    <rdfs:comment>Output only. The timestamp when the resource was updated.</rdfs:comment>
    <rdfs:domain rdf:resource="http://example.org/onto/class/google_network_services_wasm_plugin"/>
    <rdfs:range rdf:resource="http://www.w3.org/2001/XMLSchema#string"/>
  </owl:DatatypeProperty>
  <owl:DatatypeProperty rdf:about="http://example.org/onto/prop/google_network_services_wasm_plugin_used_by">
    <rdfs:label>used_by</rdfs:label>
    <rdfs:comment>Output only. List of all extensions that use this WasmPlugin resource.</rdfs:comment>
    <rdfs:domain rdf:resource="http://example.org/onto/class/google_network_services_wasm_plugin"/>
    <rdfs:range rdf:resource="http://www.w3.org/2001/XMLSchema#string"/>
  </owl:DatatypeProperty>
  <owl:DatatypeProperty rdf:about="http://example.org/onto/prop/google_network_services_wasm_plugin_enable">
    <rdfs:label>enable</rdfs:label>
    <rdfs:comment>Optional. Specifies whether to enable logging for activity by this plugin.</rdfs:comment>
    <rdfs:domain rdf:resource="http://example.org/onto/class/google_network_services_wasm_plugin"/>
    <rdfs:range rdf:resource="http://www.w3.org/2001/XMLSchema#string"/>
  </owl:DatatypeProperty>
  <owl:DatatypeProperty rdf:about="http://example.org/onto/prop/google_network_services_wasm_plugin_min_log_level">
    <rdfs:label>min_log_level</rdfs:label>
    <rdfs:comment>Non-empty default. Specificies the lowest level of the plugin logs that are exported to Cloud Logging. This setting relates to the logs generated by using logging statements in your Wasm code.
This field is can be set only if logging is enabled for the plugin.
If the field is not provided when logging is enabled, it is set to INFO by default. Possible values: ["LOG_LEVEL_UNSPECIFIED", "TRACE", "DEBUG", "INFO", "WARN", "ERROR", "CRITICAL"]</rdfs:comment>
    <rdfs:domain rdf:resource="http://example.org/onto/class/google_network_services_wasm_plugin"/>
    <rdfs:range rdf:resource="http://www.w3.org/2001/XMLSchema#string"/>
  </owl:DatatypeProperty>
  <owl:DatatypeProperty rdf:about="http://example.org/onto/prop/google_network_services_wasm_plugin_sample_rate">
    <rdfs:label>sample_rate</rdfs:label>
    <rdfs:comment>Non-empty default. Configures the sampling rate of activity logs, where 1.0 means all logged activity is reported and 0.0 means no activity is reported.
A floating point value between 0.0 and 1.0 indicates that a percentage of log messages is stored.
The default value when logging is enabled is 1.0. The value of the field must be between 0 and 1 (inclusive).
This field can be specified only if logging is enabled for this plugin.</rdfs:comment>
    <rdfs:domain rdf:resource="http://example.org/onto/class/google_network_services_wasm_plugin"/>
    <rdfs:range rdf:resource="http://www.w3.org/2001/XMLSchema#string"/>
  </owl:DatatypeProperty>
  <owl:DatatypeProperty rdf:about="http://example.org/onto/prop/google_network_services_wasm_plugin_create">
    <rdfs:label>create</rdfs:label>
    <rdfs:domain rdf:resource="http://example.org/onto/class/google_network_services_wasm_plugin"/>
    <rdfs:range rdf:resource="http://www.w3.org/2001/XMLSchema#string"/>
  </owl:DatatypeProperty>
  <owl:DatatypeProperty rdf:about="http://example.org/onto/prop/google_network_services_wasm_plugin_delete">
    <rdfs:label>delete</rdfs:label>
    <rdfs:domain rdf:resource="http://example.org/onto/class/google_network_services_wasm_plugin"/>
    <rdfs:range rdf:resource="http://www.w3.org/2001/XMLSchema#string"/>
  </owl:DatatypeProperty>
  <owl:DatatypeProperty rdf:about="http://example.org/onto/prop/google_network_services_wasm_plugin_update">
    <rdfs:label>update</rdfs:label>
    <rdfs:domain rdf:resource="http://example.org/onto/class/google_network_services_wasm_plugin"/>
    <rdfs:range rdf:resource="http://www.w3.org/2001/XMLSchema#string"/>
  </owl:DatatypeProperty>
  <owl:DatatypeProperty rdf:about="http://example.org/onto/prop/google_network_services_wasm_plugin_create_time">
    <rdfs:label>create_time</rdfs:label>
    <rdfs:comment>Output only. The timestamp when the resource was created.</rdfs:comment>
    <rdfs:domain rdf:resource="http://example.org/onto/class/google_network_services_wasm_plugin"/>
    <rdfs:range rdf:resource="http://www.w3.org/2001/XMLSchema#string"/>
  </owl:DatatypeProperty>
  <owl:DatatypeProperty rdf:about="http://example.org/onto/prop/google_network_services_wasm_plugin_description">
    <rdfs:label>description</rdfs:label>
    <rdfs:comment>Optional. A human-readable description of the resource.</rdfs:comment>
    <rdfs:domain rdf:resource="http://example.org/onto/class/google_network_services_wasm_plugin"/>
    <rdfs:range rdf:resource="http://www.w3.org/2001/XMLSchema#string"/>
  </owl:DatatypeProperty>
  <owl:DatatypeProperty rdf:about="http://example.org/onto/prop/google_network_services_wasm_plugin_image_digest">
    <rdfs:label>image_digest</rdfs:label>
    <rdfs:comment>Output only. The resolved digest for the image specified in the image field. The digest is resolved during the creation of WasmPluginVersion resource.
This field holds the digest value, regardless of whether a tag or digest was originally specified in the image field.</rdfs:comment>
    <rdfs:domain rdf:resource="http://example.org/onto/class/google_network_services_wasm_plugin"/>
    <rdfs:range rdf:resource="http://www.w3.org/2001/XMLSchema#string"/>
  </owl:DatatypeProperty>
  <owl:DatatypeProperty rdf:about="http://example.org/onto/prop/google_network_services_wasm_plugin_image_uri">
    <rdfs:label>image_uri</rdfs:label>
    <rdfs:comment>Optional. URI of the container image containing the plugin, stored in the Artifact Registry. When a new WasmPluginVersion resource is created, the digest of the container image is saved in the imageDigest field.
When downloading an image, the digest value is used instead of an image tag.</rdfs:comment>
    <rdfs:domain rdf:resource="http://example.org/onto/class/google_network_services_wasm_plugin"/>
    <rdfs:range rdf:resource="http://www.w3.org/2001/XMLSchema#string"/>
  </owl:DatatypeProperty>
  <owl:DatatypeProperty rdf:about="http://example.org/onto/prop/google_network_services_wasm_plugin_labels">
    <rdfs:label>labels</rdfs:label>
    <rdfs:comment>Optional. Set of labels associated with the WasmPlugin resource.</rdfs:comment>
    <rdfs:domain rdf:resource="http://example.org/onto/class/google_network_services_wasm_plugin"/>
    <rdfs:range rdf:resource="http://www.w3.org/2001/XMLSchema#string"/>
  </owl:DatatypeProperty>
  <owl:DatatypeProperty rdf:about="http://example.org/onto/prop/google_network_services_wasm_plugin_plugin_config_data">
    <rdfs:label>plugin_config_data</rdfs:label>
    <rdfs:comment>A base64-encoded string containing the configuration for the plugin. The configuration is provided to the plugin at runtime through the ON_CONFIGURE callback.
When a new WasmPluginVersion resource is created, the digest of the contents is saved in the pluginConfigDigest field.
Conflics with pluginConfigUri.</rdfs:comment>
    <rdfs:domain rdf:resource="http://example.org/onto/class/google_network_services_wasm_plugin"/>
    <rdfs:range rdf:resource="http://www.w3.org/2001/XMLSchema#string"/>
  </owl:DatatypeProperty>
  <owl:DatatypeProperty rdf:about="http://example.org/onto/prop/google_network_services_wasm_plugin_plugin_config_digest">
    <rdfs:label>plugin_config_digest</rdfs:label>
    <rdfs:comment>Output only. This field holds the digest (usually checksum) value for the plugin configuration.
The value is calculated based on the contents of pluginConfigData or the container image defined by the pluginConfigUri field.</rdfs:comment>
    <rdfs:domain rdf:resource="http://example.org/onto/class/google_network_services_wasm_plugin"/>
    <rdfs:range rdf:resource="http://www.w3.org/2001/XMLSchema#string"/>
  </owl:DatatypeProperty>
  <owl:DatatypeProperty rdf:about="http://example.org/onto/prop/google_network_services_wasm_plugin_plugin_config_uri">
    <rdfs:label>plugin_config_uri</rdfs:label>
    <rdfs:comment>URI of the plugin configuration stored in the Artifact Registry. The configuration is provided to the plugin at runtime through the ON_CONFIGURE callback.
The container image must contain only a single file with the name plugin.config.
When a new WasmPluginVersion resource is created, the digest of the container image is saved in the pluginConfigDigest field.
Conflics with pluginConfigData.</rdfs:comment>
    <rdfs:domain rdf:resource="http://example.org/onto/class/google_network_services_wasm_plugin"/>
    <rdfs:range rdf:resource="http://www.w3.org/2001/XMLSchema#string"/>
  </owl:DatatypeProperty>
  <owl:DatatypeProperty rdf:about="http://example.org/onto/prop/google_network_services_wasm_plugin_update_time">
    <rdfs:label>update_time</rdfs:label>
    <rdfs:comment>Output only. The timestamp when the resource was updated.</rdfs:comment>
    <rdfs:domain rdf:resource="http://example.org/onto/class/google_network_services_wasm_plugin"/>
    <rdfs:range rdf:resource="http://www.w3.org/2001/XMLSchema#string"/>
  </owl:DatatypeProperty>
  <owl:DatatypeProperty rdf:about="http://example.org/onto/prop/google_network_services_wasm_plugin_version_name">
    <rdfs:label>version_name</rdfs:label>
    <rdfs:domain rdf:resource="http://example.org/onto/class/google_network_services_wasm_plugin"/>
    <rdfs:range rdf:resource="http://www.w3.org/2001/XMLSchema#string"/>
  </owl:DatatypeProperty>
</rdf:RDF>
