<?xml version="1.0" encoding="UTF-8"?>
<rdf:RDF
  xmlns:rdf="http://www.w3.org/1999/02/22-rdf-syntax-ns#"
  xmlns:rdfs="http://www.w3.org/2000/01/rdf-schema#"
  xmlns:owl="http://www.w3.org/2002/07/owl#"
  xmlns:xsd="http://www.w3.org/2001/XMLSchema#"
  xml:base="http://example.org/onto/">
  <owl:Class rdf:about="http://example.org/onto/class/google_iam_workload_identity_pool_provider">
    <rdfs:label>google_iam_workload_identity_pool_provider</rdfs:label>
    <rdfs:comment>#
#     ***     AUTO GENERATED CODE    ***    Type: MMv1     ***
#
# ----------------------------------------------------------------------------
#
#     This code is generated by Magic Modules using the following:
#
#     Configuration: https:#github.com/GoogleCloudPlatform/magic-modules/tree/main/mmv1/products/iambeta/WorkloadIdentityPoolProvider.yaml
#     Template:      https:#github.com/GoogleCloudPlatform/magic-modules/tree/main/mmv1/templates/terraform/resource.html.markdown.tmpl
#
#     DO NOT EDIT this file directly. Any changes made to this file will be
#     overwritten during the next generation cycle.
#
# ----------------------------------------------------------------------------
subcategory: "Cloud IAM"
description: |-
  A configuration for an external identity provider.
---</rdfs:comment>
  </owl:Class>
  <owl:DatatypeProperty rdf:about="http://example.org/onto/prop/google_iam_workload_identity_pool_provider_attribute_condition">
    <rdfs:label>attribute_condition</rdfs:label>
    <rdfs:comment>[A Common Expression Language](https://opensource.google/projects/cel) expression, in
plain text, to restrict what otherwise valid authentication credentials issued by the
provider should not be accepted.

The expression must output a boolean representing whether to allow the federation.

The following keywords may be referenced in the expressions:
  * 'assertion': JSON representing the authentication credential issued by the provider.
  * 'google': The Google attributes mapped from the assertion in the 'attribute_mappings'.
  * 'attribute': The custom attributes mapped from the assertion in the 'attribute_mappings'.

The maximum length of the attribute condition expression is 4096 characters. If
unspecified, all valid authentication credential are accepted.

The following example shows how to only allow credentials with a mapped 'google.groups'
value of 'admins':
'''
"'admins' in google.groups"
'''</rdfs:comment>
    <rdfs:domain rdf:resource="http://example.org/onto/class/google_iam_workload_identity_pool_provider"/>
    <rdfs:range rdf:resource="http://www.w3.org/2001/XMLSchema#string"/>
  </owl:DatatypeProperty>
  <owl:DatatypeProperty rdf:about="http://example.org/onto/prop/google_iam_workload_identity_pool_provider_attribute_mapping">
    <rdfs:label>attribute_mapping</rdfs:label>
    <rdfs:comment>Maps attributes from authentication credentials issued by an external identity provider
to Google Cloud attributes, such as 'subject' and 'segment'.

Each key must be a string specifying the Google Cloud IAM attribute to map to.

The following keys are supported:
  * 'google.subject': The principal IAM is authenticating. You can reference this value
    in IAM bindings. This is also the subject that appears in Cloud Logging logs.
    Cannot exceed 127 characters.
  * 'google.groups': Groups the external identity belongs to. You can grant groups
    access to resources using an IAM 'principalSet' binding; access applies to all
    members of the group.

You can also provide custom attributes by specifying 'attribute.{custom_attribute}',
where '{custom_attribute}' is the name of the custom attribute to be mapped. You can
define a maximum of 50 custom attributes. The maximum length of a mapped attribute key
is 100 characters, and the key may only contain the characters [a-z0-9_].

You can reference these attributes in IAM policies to define fine-grained access for a
workload to Google Cloud resources. For example:
  * 'google.subject':
    'principal://iam.googleapis.com/projects/{project}/locations/{location}/workloadIdentityPools/{pool}/subject/{value}'
  * 'google.groups':
    'principalSet://iam.googleapis.com/projects/{project}/locations/{location}/workloadIdentityPools/{pool}/group/{value}'
  * 'attribute.{custom_attribute}':
    'principalSet://iam.googleapis.com/projects/{project}/locations/{location}/workloadIdentityPools/{pool}/attribute.{custom_attribute}/{value}'

Each value must be a [Common Expression Language](https://opensource.google/projects/cel)
function that maps an identity provider credential to the normalized attribute specified
by the corresponding map key.

You can use the 'assertion' keyword in the expression to access a JSON representation of
the authentication credential issued by the provider.

The maximum length of an attribute mapping expression is 2048 characters. When evaluated,
the total size of all mapped attributes must not exceed 8KB.

For AWS providers, the following rules apply:
  - If no attribute mapping is defined, the following default mapping applies:
    '''
    {
      "google.subject":"assertion.arn",
      "attribute.aws_role":
        "assertion.arn.contains('assumed-role')"
        " ? assertion.arn.extract('{account_arn}assumed-role/')"
        "   + 'assumed-role/'"
        "   + assertion.arn.extract('assumed-role/{role_name}/')"
        " : assertion.arn",
    }
    '''
  - If any custom attribute mappings are defined, they must include a mapping to the
    'google.subject' attribute.

For OIDC providers, the following rules apply:
  - Custom attribute mappings must be defined, and must include a mapping to the
    'google.subject' attribute. For example, the following maps the 'sub' claim of the
    incoming credential to the 'subject' attribute on a Google token.
    '''
    {"google.subject": "assertion.sub"}
    '''</rdfs:comment>
    <rdfs:domain rdf:resource="http://example.org/onto/class/google_iam_workload_identity_pool_provider"/>
    <rdfs:range rdf:resource="http://www.w3.org/2001/XMLSchema#string"/>
  </owl:DatatypeProperty>
  <owl:DatatypeProperty rdf:about="http://example.org/onto/prop/google_iam_workload_identity_pool_provider_description">
    <rdfs:label>description</rdfs:label>
    <rdfs:comment>A description for the provider. Cannot exceed 256 characters.</rdfs:comment>
    <rdfs:domain rdf:resource="http://example.org/onto/class/google_iam_workload_identity_pool_provider"/>
    <rdfs:range rdf:resource="http://www.w3.org/2001/XMLSchema#string"/>
  </owl:DatatypeProperty>
  <owl:DatatypeProperty rdf:about="http://example.org/onto/prop/google_iam_workload_identity_pool_provider_disabled">
    <rdfs:label>disabled</rdfs:label>
    <rdfs:comment>Whether the provider is disabled. You cannot use a disabled provider to exchange tokens.
However, existing tokens still grant access.</rdfs:comment>
    <rdfs:domain rdf:resource="http://example.org/onto/class/google_iam_workload_identity_pool_provider"/>
    <rdfs:range rdf:resource="http://www.w3.org/2001/XMLSchema#string"/>
  </owl:DatatypeProperty>
  <owl:DatatypeProperty rdf:about="http://example.org/onto/prop/google_iam_workload_identity_pool_provider_display_name">
    <rdfs:label>display_name</rdfs:label>
    <rdfs:comment>A display name for the provider. Cannot exceed 32 characters.</rdfs:comment>
    <rdfs:domain rdf:resource="http://example.org/onto/class/google_iam_workload_identity_pool_provider"/>
    <rdfs:range rdf:resource="http://www.w3.org/2001/XMLSchema#string"/>
  </owl:DatatypeProperty>
  <owl:DatatypeProperty rdf:about="http://example.org/onto/prop/google_iam_workload_identity_pool_provider_id">
    <rdfs:label>id</rdfs:label>
    <rdfs:domain rdf:resource="http://example.org/onto/class/google_iam_workload_identity_pool_provider"/>
    <rdfs:range rdf:resource="http://www.w3.org/2001/XMLSchema#string"/>
  </owl:DatatypeProperty>
  <owl:DatatypeProperty rdf:about="http://example.org/onto/prop/google_iam_workload_identity_pool_provider_name">
    <rdfs:label>name</rdfs:label>
    <rdfs:comment>The resource name of the provider as
'projects/{project_number}/locations/global/workloadIdentityPools/{workload_identity_pool_id}/providers/{workload_identity_pool_provider_id}'.</rdfs:comment>
    <rdfs:domain rdf:resource="http://example.org/onto/class/google_iam_workload_identity_pool_provider"/>
    <rdfs:range rdf:resource="http://www.w3.org/2001/XMLSchema#string"/>
  </owl:DatatypeProperty>
  <owl:DatatypeProperty rdf:about="http://example.org/onto/prop/google_iam_workload_identity_pool_provider_project">
    <rdfs:label>project</rdfs:label>
    <rdfs:domain rdf:resource="http://example.org/onto/class/google_iam_workload_identity_pool_provider"/>
    <rdfs:range rdf:resource="http://www.w3.org/2001/XMLSchema#string"/>
  </owl:DatatypeProperty>
  <owl:DatatypeProperty rdf:about="http://example.org/onto/prop/google_iam_workload_identity_pool_provider_state">
    <rdfs:label>state</rdfs:label>
    <rdfs:comment>The state of the provider.
* STATE_UNSPECIFIED: State unspecified.
* ACTIVE: The provider is active, and may be used to validate authentication credentials.
* DELETED: The provider is soft-deleted. Soft-deleted providers are permanently deleted
  after approximately 30 days. You can restore a soft-deleted provider using
  UndeleteWorkloadIdentityPoolProvider. You cannot reuse the ID of a soft-deleted provider
  until it is permanently deleted.</rdfs:comment>
    <rdfs:domain rdf:resource="http://example.org/onto/class/google_iam_workload_identity_pool_provider"/>
    <rdfs:range rdf:resource="http://www.w3.org/2001/XMLSchema#string"/>
  </owl:DatatypeProperty>
  <owl:DatatypeProperty rdf:about="http://example.org/onto/prop/google_iam_workload_identity_pool_provider_workload_identity_pool_id">
    <rdfs:label>workload_identity_pool_id</rdfs:label>
    <rdfs:comment>The ID used for the pool, which is the final component of the pool resource name. This
value should be 4-32 characters, and may contain the characters [a-z0-9-]. The prefix
'gcp-' is reserved for use by Google, and may not be specified.</rdfs:comment>
    <rdfs:domain rdf:resource="http://example.org/onto/class/google_iam_workload_identity_pool_provider"/>
    <rdfs:range rdf:resource="http://www.w3.org/2001/XMLSchema#string"/>
  </owl:DatatypeProperty>
  <owl:DatatypeProperty rdf:about="http://example.org/onto/prop/google_iam_workload_identity_pool_provider_workload_identity_pool_provider_id">
    <rdfs:label>workload_identity_pool_provider_id</rdfs:label>
    <rdfs:comment>The ID for the provider, which becomes the final component of the resource name. This
value must be 4-32 characters, and may contain the characters [a-z0-9-]. The prefix
'gcp-' is reserved for use by Google, and may not be specified.</rdfs:comment>
    <rdfs:domain rdf:resource="http://example.org/onto/class/google_iam_workload_identity_pool_provider"/>
    <rdfs:range rdf:resource="http://www.w3.org/2001/XMLSchema#string"/>
  </owl:DatatypeProperty>
  <owl:DatatypeProperty rdf:about="http://example.org/onto/prop/google_iam_workload_identity_pool_provider_account_id">
    <rdfs:label>account_id</rdfs:label>
    <rdfs:comment>The AWS account ID.</rdfs:comment>
    <rdfs:domain rdf:resource="http://example.org/onto/class/google_iam_workload_identity_pool_provider"/>
    <rdfs:range rdf:resource="http://www.w3.org/2001/XMLSchema#string"/>
  </owl:DatatypeProperty>
  <owl:DatatypeProperty rdf:about="http://example.org/onto/prop/google_iam_workload_identity_pool_provider_allowed_audiences">
    <rdfs:label>allowed_audiences</rdfs:label>
    <rdfs:comment>Acceptable values for the 'aud' field (audience) in the OIDC token. Token exchange
requests are rejected if the token audience does not match one of the configured
values. Each audience may be at most 256 characters. A maximum of 10 audiences may
be configured.

If this list is empty, the OIDC token audience must be equal to the full canonical
resource name of the WorkloadIdentityPoolProvider, with or without the HTTPS prefix.
For example:
'''
//iam.googleapis.com/projects/<project-number>/locations/<location>/workloadIdentityPools/<pool-id>/providers/<provider-id>
https://iam.googleapis.com/projects/<project-number>/locations/<location>/workloadIdentityPools/<pool-id>/providers/<provider-id>
'''</rdfs:comment>
    <rdfs:domain rdf:resource="http://example.org/onto/class/google_iam_workload_identity_pool_provider"/>
    <rdfs:range rdf:resource="http://www.w3.org/2001/XMLSchema#string"/>
  </owl:DatatypeProperty>
  <owl:DatatypeProperty rdf:about="http://example.org/onto/prop/google_iam_workload_identity_pool_provider_issuer_uri">
    <rdfs:label>issuer_uri</rdfs:label>
    <rdfs:comment>The OIDC issuer URL.</rdfs:comment>
    <rdfs:domain rdf:resource="http://example.org/onto/class/google_iam_workload_identity_pool_provider"/>
    <rdfs:range rdf:resource="http://www.w3.org/2001/XMLSchema#string"/>
  </owl:DatatypeProperty>
  <owl:DatatypeProperty rdf:about="http://example.org/onto/prop/google_iam_workload_identity_pool_provider_jwks_json">
    <rdfs:label>jwks_json</rdfs:label>
    <rdfs:comment>OIDC JWKs in JSON String format. For details on definition of a
JWK, see https:tools.ietf.org/html/rfc7517. If not set, then we
use the 'jwks_uri' from the discovery document fetched from the
.well-known path for the 'issuer_uri'. Currently, RSA and EC asymmetric
keys are supported. The JWK must use following format and include only
the following fields:
'''
{
  "keys": [
    {
          "kty": "RSA/EC",
          "alg": "<algorithm>",
          "use": "sig",
          "kid": "<key-id>",
          "n": "",
          "e": "",
          "x": "",
          "y": "",
          "crv": ""
    }
  ]
}
'''</rdfs:comment>
    <rdfs:domain rdf:resource="http://example.org/onto/class/google_iam_workload_identity_pool_provider"/>
    <rdfs:range rdf:resource="http://www.w3.org/2001/XMLSchema#string"/>
  </owl:DatatypeProperty>
  <owl:DatatypeProperty rdf:about="http://example.org/onto/prop/google_iam_workload_identity_pool_provider_idp_metadata_xml">
    <rdfs:label>idp_metadata_xml</rdfs:label>
    <rdfs:comment>SAML Identity provider configuration metadata xml doc.</rdfs:comment>
    <rdfs:domain rdf:resource="http://example.org/onto/class/google_iam_workload_identity_pool_provider"/>
    <rdfs:range rdf:resource="http://www.w3.org/2001/XMLSchema#string"/>
  </owl:DatatypeProperty>
  <owl:DatatypeProperty rdf:about="http://example.org/onto/prop/google_iam_workload_identity_pool_provider_create">
    <rdfs:label>create</rdfs:label>
    <rdfs:domain rdf:resource="http://example.org/onto/class/google_iam_workload_identity_pool_provider"/>
    <rdfs:range rdf:resource="http://www.w3.org/2001/XMLSchema#string"/>
  </owl:DatatypeProperty>
  <owl:DatatypeProperty rdf:about="http://example.org/onto/prop/google_iam_workload_identity_pool_provider_delete">
    <rdfs:label>delete</rdfs:label>
    <rdfs:domain rdf:resource="http://example.org/onto/class/google_iam_workload_identity_pool_provider"/>
    <rdfs:range rdf:resource="http://www.w3.org/2001/XMLSchema#string"/>
  </owl:DatatypeProperty>
  <owl:DatatypeProperty rdf:about="http://example.org/onto/prop/google_iam_workload_identity_pool_provider_update">
    <rdfs:label>update</rdfs:label>
    <rdfs:domain rdf:resource="http://example.org/onto/class/google_iam_workload_identity_pool_provider"/>
    <rdfs:range rdf:resource="http://www.w3.org/2001/XMLSchema#string"/>
  </owl:DatatypeProperty>
  <owl:DatatypeProperty rdf:about="http://example.org/onto/prop/google_iam_workload_identity_pool_provider_pem_certificate">
    <rdfs:label>pem_certificate</rdfs:label>
    <rdfs:comment>PEM certificate of the PKI used for validation. Must only contain one
ca certificate(either root or intermediate cert).</rdfs:comment>
    <rdfs:domain rdf:resource="http://example.org/onto/class/google_iam_workload_identity_pool_provider"/>
    <rdfs:range rdf:resource="http://www.w3.org/2001/XMLSchema#string"/>
  </owl:DatatypeProperty>
  <owl:DatatypeProperty rdf:about="http://example.org/onto/prop/google_iam_workload_identity_pool_provider_pem_certificate">
    <rdfs:label>pem_certificate</rdfs:label>
    <rdfs:comment>PEM certificate of the PKI used for validation. Must only contain one
ca certificate(either root or intermediate cert).</rdfs:comment>
    <rdfs:domain rdf:resource="http://example.org/onto/class/google_iam_workload_identity_pool_provider"/>
    <rdfs:range rdf:resource="http://www.w3.org/2001/XMLSchema#string"/>
  </owl:DatatypeProperty>
</rdf:RDF>
