<?xml version="1.0" encoding="UTF-8"?>
<rdf:RDF
  xmlns:rdf="http://www.w3.org/1999/02/22-rdf-syntax-ns#"
  xmlns:rdfs="http://www.w3.org/2000/01/rdf-schema#"
  xmlns:owl="http://www.w3.org/2002/07/owl#"
  xmlns:xsd="http://www.w3.org/2001/XMLSchema#"
  xml:base="http://example.org/onto/">
  <owl:Class rdf:about="http://example.org/onto/class/google_vertex_ai_endpoint">
    <rdfs:label>google_vertex_ai_endpoint</rdfs:label>
    <rdfs:comment>#
#     ***     AUTO GENERATED CODE    ***    Type: MMv1     ***
#
# ----------------------------------------------------------------------------
#
#     This code is generated by Magic Modules using the following:
#
#     Configuration: https:#github.com/GoogleCloudPlatform/magic-modules/tree/main/mmv1/products/vertexai/Endpoint.yaml
#     Template:      https:#github.com/GoogleCloudPlatform/magic-modules/tree/main/mmv1/templates/terraform/resource.html.markdown.tmpl
#
#     DO NOT EDIT this file directly. Any changes made to this file will be
#     overwritten during the next generation cycle.
#
# ----------------------------------------------------------------------------
subcategory: "Vertex AI"
description: |-
  Models are deployed into it, and afterwards Endpoint is called to obtain predictions and explanations.
---</rdfs:comment>
  </owl:Class>
  <owl:DatatypeProperty rdf:about="http://example.org/onto/prop/google_vertex_ai_endpoint_create_time">
    <rdfs:label>create_time</rdfs:label>
    <rdfs:comment>Output only. Timestamp when this Endpoint was created.</rdfs:comment>
    <rdfs:domain rdf:resource="http://example.org/onto/class/google_vertex_ai_endpoint"/>
    <rdfs:range rdf:resource="http://www.w3.org/2001/XMLSchema#string"/>
  </owl:DatatypeProperty>
  <owl:DatatypeProperty rdf:about="http://example.org/onto/prop/google_vertex_ai_endpoint_dedicated_endpoint_dns">
    <rdfs:label>dedicated_endpoint_dns</rdfs:label>
    <rdfs:comment>Output only. DNS of the dedicated endpoint. Will only be populated if dedicatedEndpointEnabled is true. Format: 'https://{endpointId}.{region}-{projectNumber}.prediction.vertexai.goog'.</rdfs:comment>
    <rdfs:domain rdf:resource="http://example.org/onto/class/google_vertex_ai_endpoint"/>
    <rdfs:range rdf:resource="http://www.w3.org/2001/XMLSchema#string"/>
  </owl:DatatypeProperty>
  <owl:DatatypeProperty rdf:about="http://example.org/onto/prop/google_vertex_ai_endpoint_dedicated_endpoint_enabled">
    <rdfs:label>dedicated_endpoint_enabled</rdfs:label>
    <rdfs:comment>If true, the endpoint will be exposed through a dedicated DNS [Endpoint.dedicated_endpoint_dns]. Your request to the dedicated DNS will be isolated from other users' traffic and will have better performance and reliability. Note: Once you enabled dedicated endpoint, you won't be able to send request to the shared DNS {region}-aiplatform.googleapis.com. The limitation will be removed soon.</rdfs:comment>
    <rdfs:domain rdf:resource="http://example.org/onto/class/google_vertex_ai_endpoint"/>
    <rdfs:range rdf:resource="http://www.w3.org/2001/XMLSchema#string"/>
  </owl:DatatypeProperty>
  <owl:DatatypeProperty rdf:about="http://example.org/onto/prop/google_vertex_ai_endpoint_deployed_models">
    <rdfs:label>deployed_models</rdfs:label>
    <rdfs:comment>Output only. The models deployed in this Endpoint. To add or remove DeployedModels use EndpointService.DeployModel and EndpointService.UndeployModel respectively. Models can also be deployed and undeployed using the [Cloud Console](https://console.cloud.google.com/vertex-ai/).</rdfs:comment>
    <rdfs:domain rdf:resource="http://example.org/onto/class/google_vertex_ai_endpoint"/>
    <rdfs:range rdf:resource="http://www.w3.org/2001/XMLSchema#string"/>
  </owl:DatatypeProperty>
  <owl:DatatypeProperty rdf:about="http://example.org/onto/prop/google_vertex_ai_endpoint_description">
    <rdfs:label>description</rdfs:label>
    <rdfs:comment>The description of the Endpoint.</rdfs:comment>
    <rdfs:domain rdf:resource="http://example.org/onto/class/google_vertex_ai_endpoint"/>
    <rdfs:range rdf:resource="http://www.w3.org/2001/XMLSchema#string"/>
  </owl:DatatypeProperty>
  <owl:DatatypeProperty rdf:about="http://example.org/onto/prop/google_vertex_ai_endpoint_display_name">
    <rdfs:label>display_name</rdfs:label>
    <rdfs:comment>Required. The display name of the Endpoint. The name can be up to 128 characters long and can consist of any UTF-8 characters.</rdfs:comment>
    <rdfs:domain rdf:resource="http://example.org/onto/class/google_vertex_ai_endpoint"/>
    <rdfs:range rdf:resource="http://www.w3.org/2001/XMLSchema#string"/>
  </owl:DatatypeProperty>
  <owl:DatatypeProperty rdf:about="http://example.org/onto/prop/google_vertex_ai_endpoint_effective_labels">
    <rdfs:label>effective_labels</rdfs:label>
    <rdfs:comment>All of labels (key/value pairs) present on the resource in GCP, including the labels configured through Terraform, other clients and services.</rdfs:comment>
    <rdfs:domain rdf:resource="http://example.org/onto/class/google_vertex_ai_endpoint"/>
    <rdfs:range rdf:resource="http://www.w3.org/2001/XMLSchema#string"/>
  </owl:DatatypeProperty>
  <owl:DatatypeProperty rdf:about="http://example.org/onto/prop/google_vertex_ai_endpoint_etag">
    <rdfs:label>etag</rdfs:label>
    <rdfs:comment>Used to perform consistent read-modify-write updates. If not set, a blind "overwrite" update happens.</rdfs:comment>
    <rdfs:domain rdf:resource="http://example.org/onto/class/google_vertex_ai_endpoint"/>
    <rdfs:range rdf:resource="http://www.w3.org/2001/XMLSchema#string"/>
  </owl:DatatypeProperty>
  <owl:DatatypeProperty rdf:about="http://example.org/onto/prop/google_vertex_ai_endpoint_id">
    <rdfs:label>id</rdfs:label>
    <rdfs:domain rdf:resource="http://example.org/onto/class/google_vertex_ai_endpoint"/>
    <rdfs:range rdf:resource="http://www.w3.org/2001/XMLSchema#string"/>
  </owl:DatatypeProperty>
  <owl:DatatypeProperty rdf:about="http://example.org/onto/prop/google_vertex_ai_endpoint_labels">
    <rdfs:label>labels</rdfs:label>
    <rdfs:comment>The labels with user-defined metadata to organize your Endpoints. Label keys and values can be no longer than 64 characters (Unicode codepoints), can only contain lowercase letters, numeric characters, underscores and dashes. International characters are allowed. See https://goo.gl/xmQnxf for more information and examples of labels.

**Note**: This field is non-authoritative, and will only manage the labels present in your configuration.
Please refer to the field 'effective_labels' for all of the labels present on the resource.</rdfs:comment>
    <rdfs:domain rdf:resource="http://example.org/onto/class/google_vertex_ai_endpoint"/>
    <rdfs:range rdf:resource="http://www.w3.org/2001/XMLSchema#string"/>
  </owl:DatatypeProperty>
  <owl:DatatypeProperty rdf:about="http://example.org/onto/prop/google_vertex_ai_endpoint_location">
    <rdfs:label>location</rdfs:label>
    <rdfs:comment>The location for the resource</rdfs:comment>
    <rdfs:domain rdf:resource="http://example.org/onto/class/google_vertex_ai_endpoint"/>
    <rdfs:range rdf:resource="http://www.w3.org/2001/XMLSchema#string"/>
  </owl:DatatypeProperty>
  <owl:DatatypeProperty rdf:about="http://example.org/onto/prop/google_vertex_ai_endpoint_model_deployment_monitoring_job">
    <rdfs:label>model_deployment_monitoring_job</rdfs:label>
    <rdfs:comment>Output only. Resource name of the Model Monitoring job associated with this Endpoint if monitoring is enabled by CreateModelDeploymentMonitoringJob. Format: 'projects/{project}/locations/{location}/modelDeploymentMonitoringJobs/{model_deployment_monitoring_job}'</rdfs:comment>
    <rdfs:domain rdf:resource="http://example.org/onto/class/google_vertex_ai_endpoint"/>
    <rdfs:range rdf:resource="http://www.w3.org/2001/XMLSchema#string"/>
  </owl:DatatypeProperty>
  <owl:DatatypeProperty rdf:about="http://example.org/onto/prop/google_vertex_ai_endpoint_name">
    <rdfs:label>name</rdfs:label>
    <rdfs:comment>The resource name of the Endpoint. The name must be numeric with no leading zeros and can be at most 10 digits.</rdfs:comment>
    <rdfs:domain rdf:resource="http://example.org/onto/class/google_vertex_ai_endpoint"/>
    <rdfs:range rdf:resource="http://www.w3.org/2001/XMLSchema#string"/>
  </owl:DatatypeProperty>
  <owl:DatatypeProperty rdf:about="http://example.org/onto/prop/google_vertex_ai_endpoint_network">
    <rdfs:label>network</rdfs:label>
    <rdfs:comment>The full name of the Google Compute Engine [network](https://cloud.google.com//compute/docs/networks-and-firewalls#networks) to which the Endpoint should be peered. Private services access must already be configured for the network. If left unspecified, the Endpoint is not peered with any network. Only one of the fields, network or enable_private_service_connect, can be set. [Format](https://cloud.google.com/compute/docs/reference/rest/v1/networks/insert): 'projects/{project}/global/networks/{network}'. Where '{project}' is a project number, as in '12345', and '{network}' is network name. Only one of the fields, 'network' or 'privateServiceConnectConfig', can be set.</rdfs:comment>
    <rdfs:domain rdf:resource="http://example.org/onto/class/google_vertex_ai_endpoint"/>
    <rdfs:range rdf:resource="http://www.w3.org/2001/XMLSchema#string"/>
  </owl:DatatypeProperty>
  <owl:DatatypeProperty rdf:about="http://example.org/onto/prop/google_vertex_ai_endpoint_project">
    <rdfs:label>project</rdfs:label>
    <rdfs:domain rdf:resource="http://example.org/onto/class/google_vertex_ai_endpoint"/>
    <rdfs:range rdf:resource="http://www.w3.org/2001/XMLSchema#string"/>
  </owl:DatatypeProperty>
  <owl:DatatypeProperty rdf:about="http://example.org/onto/prop/google_vertex_ai_endpoint_region">
    <rdfs:label>region</rdfs:label>
    <rdfs:comment>The region for the resource</rdfs:comment>
    <rdfs:domain rdf:resource="http://example.org/onto/class/google_vertex_ai_endpoint"/>
    <rdfs:range rdf:resource="http://www.w3.org/2001/XMLSchema#string"/>
  </owl:DatatypeProperty>
  <owl:DatatypeProperty rdf:about="http://example.org/onto/prop/google_vertex_ai_endpoint_terraform_labels">
    <rdfs:label>terraform_labels</rdfs:label>
    <rdfs:comment>The combination of labels configured directly on the resource
 and default labels configured on the provider.</rdfs:comment>
    <rdfs:domain rdf:resource="http://example.org/onto/class/google_vertex_ai_endpoint"/>
    <rdfs:range rdf:resource="http://www.w3.org/2001/XMLSchema#string"/>
  </owl:DatatypeProperty>
  <owl:DatatypeProperty rdf:about="http://example.org/onto/prop/google_vertex_ai_endpoint_traffic_split">
    <rdfs:label>traffic_split</rdfs:label>
    <rdfs:comment>A map from a DeployedModel's id to the percentage of this Endpoint's traffic that should be forwarded to that DeployedModel.
If a DeployedModel's id is not listed in this map, then it receives no traffic.
The traffic percentage values must add up to 100, or map must be empty if the Endpoint is to not accept any traffic at a moment. See
the 'deployModel' [example](https://cloud.google.com/vertex-ai/docs/general/deployment#deploy_a_model_to_an_endpoint) and
[documentation](https://cloud.google.com/vertex-ai/docs/reference/rest/v1beta1/projects.locations.endpoints/deployModel) for more information.

~> **Note:** To set the map to empty, set '"{}"', apply, and then remove the field from your config.</rdfs:comment>
    <rdfs:domain rdf:resource="http://example.org/onto/class/google_vertex_ai_endpoint"/>
    <rdfs:range rdf:resource="http://www.w3.org/2001/XMLSchema#string"/>
  </owl:DatatypeProperty>
  <owl:DatatypeProperty rdf:about="http://example.org/onto/prop/google_vertex_ai_endpoint_update_time">
    <rdfs:label>update_time</rdfs:label>
    <rdfs:comment>Output only. Timestamp when this Endpoint was last updated.</rdfs:comment>
    <rdfs:domain rdf:resource="http://example.org/onto/class/google_vertex_ai_endpoint"/>
    <rdfs:range rdf:resource="http://www.w3.org/2001/XMLSchema#string"/>
  </owl:DatatypeProperty>
  <owl:DatatypeProperty rdf:about="http://example.org/onto/prop/google_vertex_ai_endpoint_kms_key_name">
    <rdfs:label>kms_key_name</rdfs:label>
    <rdfs:comment>Required. The Cloud KMS resource identifier of the customer managed encryption key used to protect a resource. Has the form: 'projects/my-project/locations/my-region/keyRings/my-kr/cryptoKeys/my-key'. The key needs to be in the same region as where the compute resource is created.</rdfs:comment>
    <rdfs:domain rdf:resource="http://example.org/onto/class/google_vertex_ai_endpoint"/>
    <rdfs:range rdf:resource="http://www.w3.org/2001/XMLSchema#string"/>
  </owl:DatatypeProperty>
  <owl:DatatypeProperty rdf:about="http://example.org/onto/prop/google_vertex_ai_endpoint_enabled">
    <rdfs:label>enabled</rdfs:label>
    <rdfs:comment>If logging is enabled or not.</rdfs:comment>
    <rdfs:domain rdf:resource="http://example.org/onto/class/google_vertex_ai_endpoint"/>
    <rdfs:range rdf:resource="http://www.w3.org/2001/XMLSchema#string"/>
  </owl:DatatypeProperty>
  <owl:DatatypeProperty rdf:about="http://example.org/onto/prop/google_vertex_ai_endpoint_sampling_rate">
    <rdfs:label>sampling_rate</rdfs:label>
    <rdfs:comment>Percentage of requests to be logged, expressed as a fraction in range(0,1]</rdfs:comment>
    <rdfs:domain rdf:resource="http://example.org/onto/class/google_vertex_ai_endpoint"/>
    <rdfs:range rdf:resource="http://www.w3.org/2001/XMLSchema#string"/>
  </owl:DatatypeProperty>
  <owl:DatatypeProperty rdf:about="http://example.org/onto/prop/google_vertex_ai_endpoint_output_uri">
    <rdfs:label>output_uri</rdfs:label>
    <rdfs:comment>BigQuery URI to a project or table, up to 2000 characters long. When only the project is specified, the Dataset and Table is created. When the full table reference is specified, the Dataset must exist and table must not exist. Accepted forms: - BigQuery path. For example: 'bq://projectId' or 'bq://projectId.bqDatasetId' or 'bq://projectId.bqDatasetId.bqTableId'.</rdfs:comment>
    <rdfs:domain rdf:resource="http://example.org/onto/class/google_vertex_ai_endpoint"/>
    <rdfs:range rdf:resource="http://www.w3.org/2001/XMLSchema#string"/>
  </owl:DatatypeProperty>
  <owl:DatatypeProperty rdf:about="http://example.org/onto/prop/google_vertex_ai_endpoint_enable_private_service_connect">
    <rdfs:label>enable_private_service_connect</rdfs:label>
    <rdfs:comment>Required. If true, expose the IndexEndpoint via private service connect.</rdfs:comment>
    <rdfs:domain rdf:resource="http://example.org/onto/class/google_vertex_ai_endpoint"/>
    <rdfs:range rdf:resource="http://www.w3.org/2001/XMLSchema#string"/>
  </owl:DatatypeProperty>
  <owl:DatatypeProperty rdf:about="http://example.org/onto/prop/google_vertex_ai_endpoint_project_allowlist">
    <rdfs:label>project_allowlist</rdfs:label>
    <rdfs:comment>A list of Projects from which the forwarding rule will target the service attachment.</rdfs:comment>
    <rdfs:domain rdf:resource="http://example.org/onto/class/google_vertex_ai_endpoint"/>
    <rdfs:range rdf:resource="http://www.w3.org/2001/XMLSchema#string"/>
  </owl:DatatypeProperty>
  <owl:DatatypeProperty rdf:about="http://example.org/onto/prop/google_vertex_ai_endpoint_create">
    <rdfs:label>create</rdfs:label>
    <rdfs:domain rdf:resource="http://example.org/onto/class/google_vertex_ai_endpoint"/>
    <rdfs:range rdf:resource="http://www.w3.org/2001/XMLSchema#string"/>
  </owl:DatatypeProperty>
  <owl:DatatypeProperty rdf:about="http://example.org/onto/prop/google_vertex_ai_endpoint_delete">
    <rdfs:label>delete</rdfs:label>
    <rdfs:domain rdf:resource="http://example.org/onto/class/google_vertex_ai_endpoint"/>
    <rdfs:range rdf:resource="http://www.w3.org/2001/XMLSchema#string"/>
  </owl:DatatypeProperty>
  <owl:DatatypeProperty rdf:about="http://example.org/onto/prop/google_vertex_ai_endpoint_update">
    <rdfs:label>update</rdfs:label>
    <rdfs:domain rdf:resource="http://example.org/onto/class/google_vertex_ai_endpoint"/>
    <rdfs:range rdf:resource="http://www.w3.org/2001/XMLSchema#string"/>
  </owl:DatatypeProperty>
</rdf:RDF>
