<?xml version="1.0" encoding="UTF-8"?>
<rdf:RDF
  xmlns:rdf="http://www.w3.org/1999/02/22-rdf-syntax-ns#"
  xmlns:rdfs="http://www.w3.org/2000/01/rdf-schema#"
  xmlns:owl="http://www.w3.org/2002/07/owl#"
  xmlns:xsd="http://www.w3.org/2001/XMLSchema#"
  xml:base="http://example.org/onto/">
  <owl:Class rdf:about="http://example.org/onto/class/google_apigee_organization">
    <rdfs:label>google_apigee_organization</rdfs:label>
    <rdfs:comment>#
#     ***     AUTO GENERATED CODE    ***    Type: MMv1     ***
#
# ----------------------------------------------------------------------------
#
#     This code is generated by Magic Modules using the following:
#
#     Configuration: https:#github.com/GoogleCloudPlatform/magic-modules/tree/main/mmv1/products/apigee/Organization.yaml
#     Template:      https:#github.com/GoogleCloudPlatform/magic-modules/tree/main/mmv1/templates/terraform/resource.html.markdown.tmpl
#
#     DO NOT EDIT this file directly. Any changes made to this file will be
#     overwritten during the next generation cycle.
#
# ----------------------------------------------------------------------------
subcategory: "Apigee"
description: |-
  An `Organization` is the top-level container in Apigee.
---</rdfs:comment>
  </owl:Class>
  <owl:DatatypeProperty rdf:about="http://example.org/onto/prop/google_apigee_organization_analytics_region">
    <rdfs:label>analytics_region</rdfs:label>
    <rdfs:comment>Primary GCP region for analytics data storage. For valid values, see [Create an Apigee organization](https://cloud.google.com/apigee/docs/api-platform/get-started/create-org).</rdfs:comment>
    <rdfs:domain rdf:resource="http://example.org/onto/class/google_apigee_organization"/>
    <rdfs:range rdf:resource="http://www.w3.org/2001/XMLSchema#string"/>
  </owl:DatatypeProperty>
  <owl:DatatypeProperty rdf:about="http://example.org/onto/prop/google_apigee_organization_api_consumer_data_encryption_key_name">
    <rdfs:label>api_consumer_data_encryption_key_name</rdfs:label>
    <rdfs:comment>Cloud KMS key name used for encrypting API consumer data.</rdfs:comment>
    <rdfs:domain rdf:resource="http://example.org/onto/class/google_apigee_organization"/>
    <rdfs:range rdf:resource="http://www.w3.org/2001/XMLSchema#string"/>
  </owl:DatatypeProperty>
  <owl:DatatypeProperty rdf:about="http://example.org/onto/prop/google_apigee_organization_api_consumer_data_location">
    <rdfs:label>api_consumer_data_location</rdfs:label>
    <rdfs:comment>This field is needed only for customers using non-default data residency regions.
Apigee stores some control plane data only in single region.
This field determines which single region Apigee should use.</rdfs:comment>
    <rdfs:domain rdf:resource="http://example.org/onto/class/google_apigee_organization"/>
    <rdfs:range rdf:resource="http://www.w3.org/2001/XMLSchema#string"/>
  </owl:DatatypeProperty>
  <owl:DatatypeProperty rdf:about="http://example.org/onto/prop/google_apigee_organization_apigee_project_id">
    <rdfs:label>apigee_project_id</rdfs:label>
    <rdfs:comment>Output only. Project ID of the Apigee Tenant Project.</rdfs:comment>
    <rdfs:domain rdf:resource="http://example.org/onto/class/google_apigee_organization"/>
    <rdfs:range rdf:resource="http://www.w3.org/2001/XMLSchema#string"/>
  </owl:DatatypeProperty>
  <owl:DatatypeProperty rdf:about="http://example.org/onto/prop/google_apigee_organization_authorized_network">
    <rdfs:label>authorized_network</rdfs:label>
    <rdfs:comment>Compute Engine network used for Service Networking to be peered with Apigee runtime instances.
See [Getting started with the Service Networking API](https://cloud.google.com/service-infrastructure/docs/service-networking/getting-started).
Valid only when 'RuntimeType' is set to CLOUD. The value can be updated only when there are no runtime instances. For example: "default".</rdfs:comment>
    <rdfs:domain rdf:resource="http://example.org/onto/class/google_apigee_organization"/>
    <rdfs:range rdf:resource="http://www.w3.org/2001/XMLSchema#string"/>
  </owl:DatatypeProperty>
  <owl:DatatypeProperty rdf:about="http://example.org/onto/prop/google_apigee_organization_billing_type">
    <rdfs:label>billing_type</rdfs:label>
    <rdfs:comment>Billing type of the Apigee organization. See [Apigee pricing](https://cloud.google.com/apigee/pricing).</rdfs:comment>
    <rdfs:domain rdf:resource="http://example.org/onto/class/google_apigee_organization"/>
    <rdfs:range rdf:resource="http://www.w3.org/2001/XMLSchema#string"/>
  </owl:DatatypeProperty>
  <owl:DatatypeProperty rdf:about="http://example.org/onto/prop/google_apigee_organization_ca_certificate">
    <rdfs:label>ca_certificate</rdfs:label>
    <rdfs:comment>Output only. Base64-encoded public certificate for the root CA of the Apigee organization.
Valid only when 'RuntimeType' is CLOUD. A base64-encoded string.</rdfs:comment>
    <rdfs:domain rdf:resource="http://example.org/onto/class/google_apigee_organization"/>
    <rdfs:range rdf:resource="http://www.w3.org/2001/XMLSchema#string"/>
  </owl:DatatypeProperty>
  <owl:DatatypeProperty rdf:about="http://example.org/onto/prop/google_apigee_organization_control_plane_encryption_key_name">
    <rdfs:label>control_plane_encryption_key_name</rdfs:label>
    <rdfs:comment>Cloud KMS key name used for encrypting control plane data that is stored in a multi region.
Only used for the data residency region "US" or "EU".</rdfs:comment>
    <rdfs:domain rdf:resource="http://example.org/onto/class/google_apigee_organization"/>
    <rdfs:range rdf:resource="http://www.w3.org/2001/XMLSchema#string"/>
  </owl:DatatypeProperty>
  <owl:DatatypeProperty rdf:about="http://example.org/onto/prop/google_apigee_organization_description">
    <rdfs:label>description</rdfs:label>
    <rdfs:comment>Description of the Apigee organization.</rdfs:comment>
    <rdfs:domain rdf:resource="http://example.org/onto/class/google_apigee_organization"/>
    <rdfs:range rdf:resource="http://www.w3.org/2001/XMLSchema#string"/>
  </owl:DatatypeProperty>
  <owl:DatatypeProperty rdf:about="http://example.org/onto/prop/google_apigee_organization_disable_vpc_peering">
    <rdfs:label>disable_vpc_peering</rdfs:label>
    <rdfs:comment>Flag that specifies whether the VPC Peering through Private Google Access should be
disabled between the consumer network and Apigee. Required if an 'authorizedNetwork'
on the consumer project is not provided, in which case the flag should be set to 'true'.
Valid only when 'RuntimeType' is set to CLOUD. The value must be set before the creation
of any Apigee runtime instance and can be updated only when there are no runtime instances.</rdfs:comment>
    <rdfs:domain rdf:resource="http://example.org/onto/class/google_apigee_organization"/>
    <rdfs:range rdf:resource="http://www.w3.org/2001/XMLSchema#string"/>
  </owl:DatatypeProperty>
  <owl:DatatypeProperty rdf:about="http://example.org/onto/prop/google_apigee_organization_display_name">
    <rdfs:label>display_name</rdfs:label>
    <rdfs:comment>The display name of the Apigee organization.</rdfs:comment>
    <rdfs:domain rdf:resource="http://example.org/onto/class/google_apigee_organization"/>
    <rdfs:range rdf:resource="http://www.w3.org/2001/XMLSchema#string"/>
  </owl:DatatypeProperty>
  <owl:DatatypeProperty rdf:about="http://example.org/onto/prop/google_apigee_organization_id">
    <rdfs:label>id</rdfs:label>
    <rdfs:domain rdf:resource="http://example.org/onto/class/google_apigee_organization"/>
    <rdfs:range rdf:resource="http://www.w3.org/2001/XMLSchema#string"/>
  </owl:DatatypeProperty>
  <owl:DatatypeProperty rdf:about="http://example.org/onto/prop/google_apigee_organization_name">
    <rdfs:label>name</rdfs:label>
    <rdfs:comment>Output only. Name of the Apigee organization.</rdfs:comment>
    <rdfs:domain rdf:resource="http://example.org/onto/class/google_apigee_organization"/>
    <rdfs:range rdf:resource="http://www.w3.org/2001/XMLSchema#string"/>
  </owl:DatatypeProperty>
  <owl:DatatypeProperty rdf:about="http://example.org/onto/prop/google_apigee_organization_project_id">
    <rdfs:label>project_id</rdfs:label>
    <rdfs:comment>The project ID associated with the Apigee organization.</rdfs:comment>
    <rdfs:domain rdf:resource="http://example.org/onto/class/google_apigee_organization"/>
    <rdfs:range rdf:resource="http://www.w3.org/2001/XMLSchema#string"/>
  </owl:DatatypeProperty>
  <owl:DatatypeProperty rdf:about="http://example.org/onto/prop/google_apigee_organization_retention">
    <rdfs:label>retention</rdfs:label>
    <rdfs:comment>Optional. This setting is applicable only for organizations that are soft-deleted (i.e., BillingType
is not EVALUATION). It controls how long Organization data will be retained after the initial delete
operation completes. During this period, the Organization may be restored to its last known state.
After this period, the Organization will no longer be able to be restored. Default value: "DELETION_RETENTION_UNSPECIFIED" Possible values: ["DELETION_RETENTION_UNSPECIFIED", "MINIMUM"]</rdfs:comment>
    <rdfs:domain rdf:resource="http://example.org/onto/class/google_apigee_organization"/>
    <rdfs:range rdf:resource="http://www.w3.org/2001/XMLSchema#string"/>
  </owl:DatatypeProperty>
  <owl:DatatypeProperty rdf:about="http://example.org/onto/prop/google_apigee_organization_runtime_database_encryption_key_name">
    <rdfs:label>runtime_database_encryption_key_name</rdfs:label>
    <rdfs:comment>Cloud KMS key name used for encrypting the data that is stored and replicated across runtime instances.
Update is not allowed after the organization is created.
If not specified, a Google-Managed encryption key will be used.
Valid only when 'RuntimeType' is CLOUD. For example: 'projects/foo/locations/us/keyRings/bar/cryptoKeys/baz'.</rdfs:comment>
    <rdfs:domain rdf:resource="http://example.org/onto/class/google_apigee_organization"/>
    <rdfs:range rdf:resource="http://www.w3.org/2001/XMLSchema#string"/>
  </owl:DatatypeProperty>
  <owl:DatatypeProperty rdf:about="http://example.org/onto/prop/google_apigee_organization_runtime_type">
    <rdfs:label>runtime_type</rdfs:label>
    <rdfs:comment>Runtime type of the Apigee organization based on the Apigee subscription purchased. Default value: "CLOUD" Possible values: ["CLOUD", "HYBRID"]</rdfs:comment>
    <rdfs:domain rdf:resource="http://example.org/onto/class/google_apigee_organization"/>
    <rdfs:range rdf:resource="http://www.w3.org/2001/XMLSchema#string"/>
  </owl:DatatypeProperty>
  <owl:DatatypeProperty rdf:about="http://example.org/onto/prop/google_apigee_organization_subscription_type">
    <rdfs:label>subscription_type</rdfs:label>
    <rdfs:comment>Output only. Subscription type of the Apigee organization.
Valid values include trial (free, limited, and for evaluation purposes only) or paid (full subscription has been purchased).</rdfs:comment>
    <rdfs:domain rdf:resource="http://example.org/onto/class/google_apigee_organization"/>
    <rdfs:range rdf:resource="http://www.w3.org/2001/XMLSchema#string"/>
  </owl:DatatypeProperty>
  <owl:DatatypeProperty rdf:about="http://example.org/onto/prop/google_apigee_organization_name">
    <rdfs:label>name</rdfs:label>
    <rdfs:comment>Name of the property.</rdfs:comment>
    <rdfs:domain rdf:resource="http://example.org/onto/class/google_apigee_organization"/>
    <rdfs:range rdf:resource="http://www.w3.org/2001/XMLSchema#string"/>
  </owl:DatatypeProperty>
  <owl:DatatypeProperty rdf:about="http://example.org/onto/prop/google_apigee_organization_value">
    <rdfs:label>value</rdfs:label>
    <rdfs:comment>Value of the property.</rdfs:comment>
    <rdfs:domain rdf:resource="http://example.org/onto/class/google_apigee_organization"/>
    <rdfs:range rdf:resource="http://www.w3.org/2001/XMLSchema#string"/>
  </owl:DatatypeProperty>
  <owl:DatatypeProperty rdf:about="http://example.org/onto/prop/google_apigee_organization_create">
    <rdfs:label>create</rdfs:label>
    <rdfs:domain rdf:resource="http://example.org/onto/class/google_apigee_organization"/>
    <rdfs:range rdf:resource="http://www.w3.org/2001/XMLSchema#string"/>
  </owl:DatatypeProperty>
  <owl:DatatypeProperty rdf:about="http://example.org/onto/prop/google_apigee_organization_delete">
    <rdfs:label>delete</rdfs:label>
    <rdfs:domain rdf:resource="http://example.org/onto/class/google_apigee_organization"/>
    <rdfs:range rdf:resource="http://www.w3.org/2001/XMLSchema#string"/>
  </owl:DatatypeProperty>
  <owl:DatatypeProperty rdf:about="http://example.org/onto/prop/google_apigee_organization_update">
    <rdfs:label>update</rdfs:label>
    <rdfs:domain rdf:resource="http://example.org/onto/class/google_apigee_organization"/>
    <rdfs:range rdf:resource="http://www.w3.org/2001/XMLSchema#string"/>
  </owl:DatatypeProperty>
</rdf:RDF>
