<?xml version="1.0" encoding="UTF-8"?>
<rdf:RDF
  xmlns:rdf="http://www.w3.org/1999/02/22-rdf-syntax-ns#"
  xmlns:rdfs="http://www.w3.org/2000/01/rdf-schema#"
  xmlns:owl="http://www.w3.org/2002/07/owl#"
  xmlns:xsd="http://www.w3.org/2001/XMLSchema#"
  xml:base="http://example.org/onto/">
  <owl:Class rdf:about="http://example.org/onto/class/google_identity_platform_config">
    <rdfs:label>google_identity_platform_config</rdfs:label>
    <rdfs:comment>#
#     ***     AUTO GENERATED CODE    ***    Type: MMv1     ***
#
# ----------------------------------------------------------------------------
#
#     This code is generated by Magic Modules using the following:
#
#     Configuration: https:#github.com/GoogleCloudPlatform/magic-modules/tree/main/mmv1/products/identityplatform/Config.yaml
#     Template:      https:#github.com/GoogleCloudPlatform/magic-modules/tree/main/mmv1/templates/terraform/resource.html.markdown.tmpl
#
#     DO NOT EDIT this file directly. Any changes made to this file will be
#     overwritten during the next generation cycle.
#
# ----------------------------------------------------------------------------
subcategory: "Identity Platform"
description: |-
  Identity Platform configuration for a Cloud project.
---</rdfs:comment>
  </owl:Class>
  <owl:DatatypeProperty rdf:about="http://example.org/onto/prop/google_identity_platform_config_authorized_domains">
    <rdfs:label>authorized_domains</rdfs:label>
    <rdfs:comment>List of domains authorized for OAuth redirects.</rdfs:comment>
    <rdfs:domain rdf:resource="http://example.org/onto/class/google_identity_platform_config"/>
    <rdfs:range rdf:resource="http://www.w3.org/2001/XMLSchema#string"/>
  </owl:DatatypeProperty>
  <owl:DatatypeProperty rdf:about="http://example.org/onto/prop/google_identity_platform_config_autodelete_anonymous_users">
    <rdfs:label>autodelete_anonymous_users</rdfs:label>
    <rdfs:comment>Whether anonymous users will be auto-deleted after a period of 30 days</rdfs:comment>
    <rdfs:domain rdf:resource="http://example.org/onto/class/google_identity_platform_config"/>
    <rdfs:range rdf:resource="http://www.w3.org/2001/XMLSchema#string"/>
  </owl:DatatypeProperty>
  <owl:DatatypeProperty rdf:about="http://example.org/onto/prop/google_identity_platform_config_id">
    <rdfs:label>id</rdfs:label>
    <rdfs:domain rdf:resource="http://example.org/onto/class/google_identity_platform_config"/>
    <rdfs:range rdf:resource="http://www.w3.org/2001/XMLSchema#string"/>
  </owl:DatatypeProperty>
  <owl:DatatypeProperty rdf:about="http://example.org/onto/prop/google_identity_platform_config_name">
    <rdfs:label>name</rdfs:label>
    <rdfs:comment>The name of the Config resource</rdfs:comment>
    <rdfs:domain rdf:resource="http://example.org/onto/class/google_identity_platform_config"/>
    <rdfs:range rdf:resource="http://www.w3.org/2001/XMLSchema#string"/>
  </owl:DatatypeProperty>
  <owl:DatatypeProperty rdf:about="http://example.org/onto/prop/google_identity_platform_config_project">
    <rdfs:label>project</rdfs:label>
    <rdfs:domain rdf:resource="http://example.org/onto/class/google_identity_platform_config"/>
    <rdfs:range rdf:resource="http://www.w3.org/2001/XMLSchema#string"/>
  </owl:DatatypeProperty>
  <owl:DatatypeProperty rdf:about="http://example.org/onto/prop/google_identity_platform_config_access_token">
    <rdfs:label>access_token</rdfs:label>
    <rdfs:comment>Whether to pass the user's OAuth identity provider's access token.</rdfs:comment>
    <rdfs:domain rdf:resource="http://example.org/onto/class/google_identity_platform_config"/>
    <rdfs:range rdf:resource="http://www.w3.org/2001/XMLSchema#string"/>
  </owl:DatatypeProperty>
  <owl:DatatypeProperty rdf:about="http://example.org/onto/prop/google_identity_platform_config_id_token">
    <rdfs:label>id_token</rdfs:label>
    <rdfs:comment>Whether to pass the user's OIDC identity provider's ID token.</rdfs:comment>
    <rdfs:domain rdf:resource="http://example.org/onto/class/google_identity_platform_config"/>
    <rdfs:range rdf:resource="http://www.w3.org/2001/XMLSchema#string"/>
  </owl:DatatypeProperty>
  <owl:DatatypeProperty rdf:about="http://example.org/onto/prop/google_identity_platform_config_refresh_token">
    <rdfs:label>refresh_token</rdfs:label>
    <rdfs:comment>Whether to pass the user's OAuth identity provider's refresh token.</rdfs:comment>
    <rdfs:domain rdf:resource="http://example.org/onto/class/google_identity_platform_config"/>
    <rdfs:range rdf:resource="http://www.w3.org/2001/XMLSchema#string"/>
  </owl:DatatypeProperty>
  <owl:DatatypeProperty rdf:about="http://example.org/onto/prop/google_identity_platform_config_event_type">
    <rdfs:label>event_type</rdfs:label>
    <rdfs:domain rdf:resource="http://example.org/onto/class/google_identity_platform_config"/>
    <rdfs:range rdf:resource="http://www.w3.org/2001/XMLSchema#string"/>
  </owl:DatatypeProperty>
  <owl:DatatypeProperty rdf:about="http://example.org/onto/prop/google_identity_platform_config_function_uri">
    <rdfs:label>function_uri</rdfs:label>
    <rdfs:comment>HTTP URI trigger for the Cloud Function.</rdfs:comment>
    <rdfs:domain rdf:resource="http://example.org/onto/class/google_identity_platform_config"/>
    <rdfs:range rdf:resource="http://www.w3.org/2001/XMLSchema#string"/>
  </owl:DatatypeProperty>
  <owl:DatatypeProperty rdf:about="http://example.org/onto/prop/google_identity_platform_config_update_time">
    <rdfs:label>update_time</rdfs:label>
    <rdfs:comment>When the trigger was changed.</rdfs:comment>
    <rdfs:domain rdf:resource="http://example.org/onto/class/google_identity_platform_config"/>
    <rdfs:range rdf:resource="http://www.w3.org/2001/XMLSchema#string"/>
  </owl:DatatypeProperty>
  <owl:DatatypeProperty rdf:about="http://example.org/onto/prop/google_identity_platform_config_api_key">
    <rdfs:label>api_key</rdfs:label>
    <rdfs:comment>API key that can be used when making requests for this project.</rdfs:comment>
    <rdfs:domain rdf:resource="http://example.org/onto/class/google_identity_platform_config"/>
    <rdfs:range rdf:resource="http://www.w3.org/2001/XMLSchema#string"/>
  </owl:DatatypeProperty>
  <owl:DatatypeProperty rdf:about="http://example.org/onto/prop/google_identity_platform_config_firebase_subdomain">
    <rdfs:label>firebase_subdomain</rdfs:label>
    <rdfs:comment>Firebase subdomain.</rdfs:comment>
    <rdfs:domain rdf:resource="http://example.org/onto/class/google_identity_platform_config"/>
    <rdfs:range rdf:resource="http://www.w3.org/2001/XMLSchema#string"/>
  </owl:DatatypeProperty>
  <owl:DatatypeProperty rdf:about="http://example.org/onto/prop/google_identity_platform_config_disabled_user_deletion">
    <rdfs:label>disabled_user_deletion</rdfs:label>
    <rdfs:comment>When true, end users cannot delete their account on the associated project through any of our API methods</rdfs:comment>
    <rdfs:domain rdf:resource="http://example.org/onto/class/google_identity_platform_config"/>
    <rdfs:range rdf:resource="http://www.w3.org/2001/XMLSchema#string"/>
  </owl:DatatypeProperty>
  <owl:DatatypeProperty rdf:about="http://example.org/onto/prop/google_identity_platform_config_disabled_user_signup">
    <rdfs:label>disabled_user_signup</rdfs:label>
    <rdfs:comment>When true, end users cannot sign up for a new account on the associated project through any of our API methods</rdfs:comment>
    <rdfs:domain rdf:resource="http://example.org/onto/class/google_identity_platform_config"/>
    <rdfs:range rdf:resource="http://www.w3.org/2001/XMLSchema#string"/>
  </owl:DatatypeProperty>
  <owl:DatatypeProperty rdf:about="http://example.org/onto/prop/google_identity_platform_config_enabled_providers">
    <rdfs:label>enabled_providers</rdfs:label>
    <rdfs:comment>A list of usable second factors for this project. Possible values: ["PHONE_SMS"]</rdfs:comment>
    <rdfs:domain rdf:resource="http://example.org/onto/class/google_identity_platform_config"/>
    <rdfs:range rdf:resource="http://www.w3.org/2001/XMLSchema#string"/>
  </owl:DatatypeProperty>
  <owl:DatatypeProperty rdf:about="http://example.org/onto/prop/google_identity_platform_config_state">
    <rdfs:label>state</rdfs:label>
    <rdfs:comment>Whether MultiFactor Authentication has been enabled for this project. Possible values: ["DISABLED", "ENABLED", "MANDATORY"]</rdfs:comment>
    <rdfs:domain rdf:resource="http://example.org/onto/class/google_identity_platform_config"/>
    <rdfs:range rdf:resource="http://www.w3.org/2001/XMLSchema#string"/>
  </owl:DatatypeProperty>
  <owl:DatatypeProperty rdf:about="http://example.org/onto/prop/google_identity_platform_config_state">
    <rdfs:label>state</rdfs:label>
    <rdfs:comment>Whether MultiFactor Authentication has been enabled for this project. Possible values: ["DISABLED", "ENABLED", "MANDATORY"]</rdfs:comment>
    <rdfs:domain rdf:resource="http://example.org/onto/class/google_identity_platform_config"/>
    <rdfs:range rdf:resource="http://www.w3.org/2001/XMLSchema#string"/>
  </owl:DatatypeProperty>
  <owl:DatatypeProperty rdf:about="http://example.org/onto/prop/google_identity_platform_config_adjacent_intervals">
    <rdfs:label>adjacent_intervals</rdfs:label>
    <rdfs:comment>The allowed number of adjacent intervals that will be used for verification to avoid clock skew.</rdfs:comment>
    <rdfs:domain rdf:resource="http://example.org/onto/class/google_identity_platform_config"/>
    <rdfs:range rdf:resource="http://www.w3.org/2001/XMLSchema#string"/>
  </owl:DatatypeProperty>
  <owl:DatatypeProperty rdf:about="http://example.org/onto/prop/google_identity_platform_config_enabled">
    <rdfs:label>enabled</rdfs:label>
    <rdfs:comment>Whether logging is enabled for this project or not.</rdfs:comment>
    <rdfs:domain rdf:resource="http://example.org/onto/class/google_identity_platform_config"/>
    <rdfs:range rdf:resource="http://www.w3.org/2001/XMLSchema#string"/>
  </owl:DatatypeProperty>
  <owl:DatatypeProperty rdf:about="http://example.org/onto/prop/google_identity_platform_config_allow_tenants">
    <rdfs:label>allow_tenants</rdfs:label>
    <rdfs:comment>Whether this project can have tenants or not.</rdfs:comment>
    <rdfs:domain rdf:resource="http://example.org/onto/class/google_identity_platform_config"/>
    <rdfs:range rdf:resource="http://www.w3.org/2001/XMLSchema#string"/>
  </owl:DatatypeProperty>
  <owl:DatatypeProperty rdf:about="http://example.org/onto/prop/google_identity_platform_config_default_tenant_location">
    <rdfs:label>default_tenant_location</rdfs:label>
    <rdfs:comment>The default cloud parent org or folder that the tenant project should be created under.
The parent resource name should be in the format of "/", such as "folders/123" or "organizations/456".
If the value is not set, the tenant will be created under the same organization or folder as the agent project.</rdfs:comment>
    <rdfs:domain rdf:resource="http://example.org/onto/class/google_identity_platform_config"/>
    <rdfs:range rdf:resource="http://www.w3.org/2001/XMLSchema#string"/>
  </owl:DatatypeProperty>
  <owl:DatatypeProperty rdf:about="http://example.org/onto/prop/google_identity_platform_config_quota">
    <rdfs:label>quota</rdfs:label>
    <rdfs:comment>A sign up APIs quota that customers can override temporarily. Value can be in between 1 and 1000.</rdfs:comment>
    <rdfs:domain rdf:resource="http://example.org/onto/class/google_identity_platform_config"/>
    <rdfs:range rdf:resource="http://www.w3.org/2001/XMLSchema#string"/>
  </owl:DatatypeProperty>
  <owl:DatatypeProperty rdf:about="http://example.org/onto/prop/google_identity_platform_config_quota_duration">
    <rdfs:label>quota_duration</rdfs:label>
    <rdfs:comment>How long this quota will be active for. It is measurred in seconds, e.g., Example: "9.615s".</rdfs:comment>
    <rdfs:domain rdf:resource="http://example.org/onto/class/google_identity_platform_config"/>
    <rdfs:range rdf:resource="http://www.w3.org/2001/XMLSchema#string"/>
  </owl:DatatypeProperty>
  <owl:DatatypeProperty rdf:about="http://example.org/onto/prop/google_identity_platform_config_start_time">
    <rdfs:label>start_time</rdfs:label>
    <rdfs:comment>When this quota will take affect.</rdfs:comment>
    <rdfs:domain rdf:resource="http://example.org/onto/class/google_identity_platform_config"/>
    <rdfs:range rdf:resource="http://www.w3.org/2001/XMLSchema#string"/>
  </owl:DatatypeProperty>
  <owl:DatatypeProperty rdf:about="http://example.org/onto/prop/google_identity_platform_config_allow_duplicate_emails">
    <rdfs:label>allow_duplicate_emails</rdfs:label>
    <rdfs:comment>Whether to allow more than one account to have the same email.</rdfs:comment>
    <rdfs:domain rdf:resource="http://example.org/onto/class/google_identity_platform_config"/>
    <rdfs:range rdf:resource="http://www.w3.org/2001/XMLSchema#string"/>
  </owl:DatatypeProperty>
  <owl:DatatypeProperty rdf:about="http://example.org/onto/prop/google_identity_platform_config_hash_config">
    <rdfs:label>hash_config</rdfs:label>
    <rdfs:comment>Output only. Hash config information.</rdfs:comment>
    <rdfs:domain rdf:resource="http://example.org/onto/class/google_identity_platform_config"/>
    <rdfs:range rdf:resource="http://www.w3.org/2001/XMLSchema#string"/>
  </owl:DatatypeProperty>
  <owl:DatatypeProperty rdf:about="http://example.org/onto/prop/google_identity_platform_config_enabled">
    <rdfs:label>enabled</rdfs:label>
    <rdfs:comment>Whether anonymous user auth is enabled for the project or not.</rdfs:comment>
    <rdfs:domain rdf:resource="http://example.org/onto/class/google_identity_platform_config"/>
    <rdfs:range rdf:resource="http://www.w3.org/2001/XMLSchema#string"/>
  </owl:DatatypeProperty>
  <owl:DatatypeProperty rdf:about="http://example.org/onto/prop/google_identity_platform_config_enabled">
    <rdfs:label>enabled</rdfs:label>
    <rdfs:comment>Whether email auth is enabled for the project or not.</rdfs:comment>
    <rdfs:domain rdf:resource="http://example.org/onto/class/google_identity_platform_config"/>
    <rdfs:range rdf:resource="http://www.w3.org/2001/XMLSchema#string"/>
  </owl:DatatypeProperty>
  <owl:DatatypeProperty rdf:about="http://example.org/onto/prop/google_identity_platform_config_password_required">
    <rdfs:label>password_required</rdfs:label>
    <rdfs:comment>Whether a password is required for email auth or not. If true, both an email and
password must be provided to sign in. If false, a user may sign in via either
email/password or email link.</rdfs:comment>
    <rdfs:domain rdf:resource="http://example.org/onto/class/google_identity_platform_config"/>
    <rdfs:range rdf:resource="http://www.w3.org/2001/XMLSchema#string"/>
  </owl:DatatypeProperty>
  <owl:DatatypeProperty rdf:about="http://example.org/onto/prop/google_identity_platform_config_enabled">
    <rdfs:label>enabled</rdfs:label>
    <rdfs:comment>Whether phone number auth is enabled for the project or not.</rdfs:comment>
    <rdfs:domain rdf:resource="http://example.org/onto/class/google_identity_platform_config"/>
    <rdfs:range rdf:resource="http://www.w3.org/2001/XMLSchema#string"/>
  </owl:DatatypeProperty>
  <owl:DatatypeProperty rdf:about="http://example.org/onto/prop/google_identity_platform_config_test_phone_numbers">
    <rdfs:label>test_phone_numbers</rdfs:label>
    <rdfs:comment>A map of <test phone number, fake code> that can be used for phone auth testing.</rdfs:comment>
    <rdfs:domain rdf:resource="http://example.org/onto/class/google_identity_platform_config"/>
    <rdfs:range rdf:resource="http://www.w3.org/2001/XMLSchema#string"/>
  </owl:DatatypeProperty>
  <owl:DatatypeProperty rdf:about="http://example.org/onto/prop/google_identity_platform_config_disallowed_regions">
    <rdfs:label>disallowed_regions</rdfs:label>
    <rdfs:comment>Two letter unicode region codes to disallow as defined by https://cldr.unicode.org/ The full list of these region codes is here: https://github.com/unicode-cldr/cldr-localenames-full/blob/master/main/en/territories.json</rdfs:comment>
    <rdfs:domain rdf:resource="http://example.org/onto/class/google_identity_platform_config"/>
    <rdfs:range rdf:resource="http://www.w3.org/2001/XMLSchema#string"/>
  </owl:DatatypeProperty>
  <owl:DatatypeProperty rdf:about="http://example.org/onto/prop/google_identity_platform_config_allowed_regions">
    <rdfs:label>allowed_regions</rdfs:label>
    <rdfs:comment>Two letter unicode region codes to allow as defined by https://cldr.unicode.org/ The full list of these region codes is here: https://github.com/unicode-cldr/cldr-localenames-full/blob/master/main/en/territories.json</rdfs:comment>
    <rdfs:domain rdf:resource="http://example.org/onto/class/google_identity_platform_config"/>
    <rdfs:range rdf:resource="http://www.w3.org/2001/XMLSchema#string"/>
  </owl:DatatypeProperty>
  <owl:DatatypeProperty rdf:about="http://example.org/onto/prop/google_identity_platform_config_create">
    <rdfs:label>create</rdfs:label>
    <rdfs:domain rdf:resource="http://example.org/onto/class/google_identity_platform_config"/>
    <rdfs:range rdf:resource="http://www.w3.org/2001/XMLSchema#string"/>
  </owl:DatatypeProperty>
  <owl:DatatypeProperty rdf:about="http://example.org/onto/prop/google_identity_platform_config_delete">
    <rdfs:label>delete</rdfs:label>
    <rdfs:domain rdf:resource="http://example.org/onto/class/google_identity_platform_config"/>
    <rdfs:range rdf:resource="http://www.w3.org/2001/XMLSchema#string"/>
  </owl:DatatypeProperty>
  <owl:DatatypeProperty rdf:about="http://example.org/onto/prop/google_identity_platform_config_update">
    <rdfs:label>update</rdfs:label>
    <rdfs:domain rdf:resource="http://example.org/onto/class/google_identity_platform_config"/>
    <rdfs:range rdf:resource="http://www.w3.org/2001/XMLSchema#string"/>
  </owl:DatatypeProperty>
</rdf:RDF>
