<?xml version="1.0" encoding="UTF-8"?>
<rdf:RDF
  xmlns:rdf="http://www.w3.org/1999/02/22-rdf-syntax-ns#"
  xmlns:rdfs="http://www.w3.org/2000/01/rdf-schema#"
  xmlns:owl="http://www.w3.org/2002/07/owl#"
  xmlns:xsd="http://www.w3.org/2001/XMLSchema#"
  xml:base="http://example.org/onto/">
  <owl:Class rdf:about="http://example.org/onto/class/google_storage_notification">
    <rdfs:label>google_storage_notification</rdfs:label>
    <rdfs:comment>Creates a new notification configuration on a specified bucket, establishing a flow of event notifications from GCS to a Cloud Pub/Sub topic.</rdfs:comment>
  </owl:Class>
  <owl:DatatypeProperty rdf:about="http://example.org/onto/prop/google_storage_notification_bucket">
    <rdfs:label>bucket</rdfs:label>
    <rdfs:comment>The name of the bucket.</rdfs:comment>
    <rdfs:domain rdf:resource="http://example.org/onto/class/google_storage_notification"/>
    <rdfs:range rdf:resource="http://www.w3.org/2001/XMLSchema#string"/>
  </owl:DatatypeProperty>
  <owl:DatatypeProperty rdf:about="http://example.org/onto/prop/google_storage_notification_custom_attributes">
    <rdfs:label>custom_attributes</rdfs:label>
    <rdfs:comment>A set of key/value attribute pairs to attach to each Cloud Pub/Sub message published for this notification subscription.</rdfs:comment>
    <rdfs:domain rdf:resource="http://example.org/onto/class/google_storage_notification"/>
    <rdfs:range rdf:resource="http://www.w3.org/2001/XMLSchema#string"/>
  </owl:DatatypeProperty>
  <owl:DatatypeProperty rdf:about="http://example.org/onto/prop/google_storage_notification_event_types">
    <rdfs:label>event_types</rdfs:label>
    <rdfs:comment>List of event type filters for this notification config. If not specified, Cloud Storage will send notifications for all event types. The valid types are: "OBJECT_FINALIZE", "OBJECT_METADATA_UPDATE", "OBJECT_DELETE", "OBJECT_ARCHIVE"</rdfs:comment>
    <rdfs:domain rdf:resource="http://example.org/onto/class/google_storage_notification"/>
    <rdfs:range rdf:resource="http://www.w3.org/2001/XMLSchema#string"/>
  </owl:DatatypeProperty>
  <owl:DatatypeProperty rdf:about="http://example.org/onto/prop/google_storage_notification_id">
    <rdfs:label>id</rdfs:label>
    <rdfs:domain rdf:resource="http://example.org/onto/class/google_storage_notification"/>
    <rdfs:range rdf:resource="http://www.w3.org/2001/XMLSchema#string"/>
  </owl:DatatypeProperty>
  <owl:DatatypeProperty rdf:about="http://example.org/onto/prop/google_storage_notification_notification_id">
    <rdfs:label>notification_id</rdfs:label>
    <rdfs:comment>The ID of the created notification.</rdfs:comment>
    <rdfs:domain rdf:resource="http://example.org/onto/class/google_storage_notification"/>
    <rdfs:range rdf:resource="http://www.w3.org/2001/XMLSchema#string"/>
  </owl:DatatypeProperty>
  <owl:DatatypeProperty rdf:about="http://example.org/onto/prop/google_storage_notification_object_name_prefix">
    <rdfs:label>object_name_prefix</rdfs:label>
    <rdfs:comment>Specifies a prefix path filter for this notification config. Cloud Storage will only send notifications for objects in this bucket whose names begin with the specified prefix.</rdfs:comment>
    <rdfs:domain rdf:resource="http://example.org/onto/class/google_storage_notification"/>
    <rdfs:range rdf:resource="http://www.w3.org/2001/XMLSchema#string"/>
  </owl:DatatypeProperty>
  <owl:DatatypeProperty rdf:about="http://example.org/onto/prop/google_storage_notification_payload_format">
    <rdfs:label>payload_format</rdfs:label>
    <rdfs:comment>The desired content of the Payload. One of "JSON_API_V1" or "NONE".</rdfs:comment>
    <rdfs:domain rdf:resource="http://example.org/onto/class/google_storage_notification"/>
    <rdfs:range rdf:resource="http://www.w3.org/2001/XMLSchema#string"/>
  </owl:DatatypeProperty>
  <owl:DatatypeProperty rdf:about="http://example.org/onto/prop/google_storage_notification_self_link">
    <rdfs:label>self_link</rdfs:label>
    <rdfs:comment>The URI of the created resource.</rdfs:comment>
    <rdfs:domain rdf:resource="http://example.org/onto/class/google_storage_notification"/>
    <rdfs:range rdf:resource="http://www.w3.org/2001/XMLSchema#string"/>
  </owl:DatatypeProperty>
  <owl:DatatypeProperty rdf:about="http://example.org/onto/prop/google_storage_notification_topic">
    <rdfs:label>topic</rdfs:label>
    <rdfs:comment>The Cloud Pub/Sub topic to which this subscription publishes.</rdfs:comment>
    <rdfs:domain rdf:resource="http://example.org/onto/class/google_storage_notification"/>
    <rdfs:range rdf:resource="http://www.w3.org/2001/XMLSchema#string"/>
  </owl:DatatypeProperty>
</rdf:RDF>
