<?xml version="1.0" encoding="UTF-8"?>
<rdf:RDF
  xmlns:rdf="http://www.w3.org/1999/02/22-rdf-syntax-ns#"
  xmlns:rdfs="http://www.w3.org/2000/01/rdf-schema#"
  xmlns:owl="http://www.w3.org/2002/07/owl#"
  xmlns:xsd="http://www.w3.org/2001/XMLSchema#"
  xml:base="http://example.org/onto/">
  <owl:Class rdf:about="http://example.org/onto/class/google_kms_ekm_connection">
    <rdfs:label>google_kms_ekm_connection</rdfs:label>
    <rdfs:comment>#
#     ***     AUTO GENERATED CODE    ***    Type: MMv1     ***
#
# ----------------------------------------------------------------------------
#
#     This code is generated by Magic Modules using the following:
#
#     Configuration: https:#github.com/GoogleCloudPlatform/magic-modules/tree/main/mmv1/products/kms/EkmConnection.yaml
#     Template:      https:#github.com/GoogleCloudPlatform/magic-modules/tree/main/mmv1/templates/terraform/resource.html.markdown.tmpl
#
#     DO NOT EDIT this file directly. Any changes made to this file will be
#     overwritten during the next generation cycle.
#
# ----------------------------------------------------------------------------
subcategory: "Cloud Key Management Service"
description: |-
  `Ekm Connections` are used to control the connection settings for an `EXTERNAL_VPC` CryptoKey.
---</rdfs:comment>
  </owl:Class>
  <owl:DatatypeProperty rdf:about="http://example.org/onto/prop/google_kms_ekm_connection_create_time">
    <rdfs:label>create_time</rdfs:label>
    <rdfs:comment>Output only. The time at which the EkmConnection was created.
A timestamp in RFC3339 UTC "Zulu" format, with nanosecond resolution and up to nine fractional digits. Examples: "2014-10-02T15:01:23Z" and "2014-10-02T15:01:23.045123456Z".</rdfs:comment>
    <rdfs:domain rdf:resource="http://example.org/onto/class/google_kms_ekm_connection"/>
    <rdfs:range rdf:resource="http://www.w3.org/2001/XMLSchema#string"/>
  </owl:DatatypeProperty>
  <owl:DatatypeProperty rdf:about="http://example.org/onto/prop/google_kms_ekm_connection_crypto_space_path">
    <rdfs:label>crypto_space_path</rdfs:label>
    <rdfs:comment>Optional. Identifies the EKM Crypto Space that this EkmConnection maps to. Note: This field is required if KeyManagementMode is CLOUD_KMS.</rdfs:comment>
    <rdfs:domain rdf:resource="http://example.org/onto/class/google_kms_ekm_connection"/>
    <rdfs:range rdf:resource="http://www.w3.org/2001/XMLSchema#string"/>
  </owl:DatatypeProperty>
  <owl:DatatypeProperty rdf:about="http://example.org/onto/prop/google_kms_ekm_connection_etag">
    <rdfs:label>etag</rdfs:label>
    <rdfs:comment>Optional. Etag of the currently stored EkmConnection.</rdfs:comment>
    <rdfs:domain rdf:resource="http://example.org/onto/class/google_kms_ekm_connection"/>
    <rdfs:range rdf:resource="http://www.w3.org/2001/XMLSchema#string"/>
  </owl:DatatypeProperty>
  <owl:DatatypeProperty rdf:about="http://example.org/onto/prop/google_kms_ekm_connection_id">
    <rdfs:label>id</rdfs:label>
    <rdfs:domain rdf:resource="http://example.org/onto/class/google_kms_ekm_connection"/>
    <rdfs:range rdf:resource="http://www.w3.org/2001/XMLSchema#string"/>
  </owl:DatatypeProperty>
  <owl:DatatypeProperty rdf:about="http://example.org/onto/prop/google_kms_ekm_connection_key_management_mode">
    <rdfs:label>key_management_mode</rdfs:label>
    <rdfs:comment>Optional. Describes who can perform control plane operations on the EKM. If unset, this defaults to MANUAL Default value: "MANUAL" Possible values: ["MANUAL", "CLOUD_KMS"]</rdfs:comment>
    <rdfs:domain rdf:resource="http://example.org/onto/class/google_kms_ekm_connection"/>
    <rdfs:range rdf:resource="http://www.w3.org/2001/XMLSchema#string"/>
  </owl:DatatypeProperty>
  <owl:DatatypeProperty rdf:about="http://example.org/onto/prop/google_kms_ekm_connection_location">
    <rdfs:label>location</rdfs:label>
    <rdfs:comment>The location for the EkmConnection.
A full list of valid locations can be found by running 'gcloud kms locations list'.</rdfs:comment>
    <rdfs:domain rdf:resource="http://example.org/onto/class/google_kms_ekm_connection"/>
    <rdfs:range rdf:resource="http://www.w3.org/2001/XMLSchema#string"/>
  </owl:DatatypeProperty>
  <owl:DatatypeProperty rdf:about="http://example.org/onto/prop/google_kms_ekm_connection_name">
    <rdfs:label>name</rdfs:label>
    <rdfs:comment>The resource name for the EkmConnection.</rdfs:comment>
    <rdfs:domain rdf:resource="http://example.org/onto/class/google_kms_ekm_connection"/>
    <rdfs:range rdf:resource="http://www.w3.org/2001/XMLSchema#string"/>
  </owl:DatatypeProperty>
  <owl:DatatypeProperty rdf:about="http://example.org/onto/prop/google_kms_ekm_connection_project">
    <rdfs:label>project</rdfs:label>
    <rdfs:domain rdf:resource="http://example.org/onto/class/google_kms_ekm_connection"/>
    <rdfs:range rdf:resource="http://www.w3.org/2001/XMLSchema#string"/>
  </owl:DatatypeProperty>
  <owl:DatatypeProperty rdf:about="http://example.org/onto/prop/google_kms_ekm_connection_endpoint_filter">
    <rdfs:label>endpoint_filter</rdfs:label>
    <rdfs:comment>Optional. The filter applied to the endpoints of the resolved service. If no filter is specified, all endpoints will be considered. An endpoint will be chosen arbitrarily from the filtered list for each request. For endpoint filter syntax and examples, see https://cloud.google.com/service-directory/docs/reference/rpc/google.cloud.servicedirectory.v1#resolveservicerequest.</rdfs:comment>
    <rdfs:domain rdf:resource="http://example.org/onto/class/google_kms_ekm_connection"/>
    <rdfs:range rdf:resource="http://www.w3.org/2001/XMLSchema#string"/>
  </owl:DatatypeProperty>
  <owl:DatatypeProperty rdf:about="http://example.org/onto/prop/google_kms_ekm_connection_hostname">
    <rdfs:label>hostname</rdfs:label>
    <rdfs:comment>Required. The hostname of the EKM replica used at TLS and HTTP layers.</rdfs:comment>
    <rdfs:domain rdf:resource="http://example.org/onto/class/google_kms_ekm_connection"/>
    <rdfs:range rdf:resource="http://www.w3.org/2001/XMLSchema#string"/>
  </owl:DatatypeProperty>
  <owl:DatatypeProperty rdf:about="http://example.org/onto/prop/google_kms_ekm_connection_service_directory_service">
    <rdfs:label>service_directory_service</rdfs:label>
    <rdfs:comment>Required. The resource name of the Service Directory service pointing to an EKM replica, in the format projects/*/locations/*/namespaces/*/services/*</rdfs:comment>
    <rdfs:domain rdf:resource="http://example.org/onto/class/google_kms_ekm_connection"/>
    <rdfs:range rdf:resource="http://www.w3.org/2001/XMLSchema#string"/>
  </owl:DatatypeProperty>
  <owl:DatatypeProperty rdf:about="http://example.org/onto/prop/google_kms_ekm_connection_issuer">
    <rdfs:label>issuer</rdfs:label>
    <rdfs:comment>Output only. The issuer distinguished name in RFC 2253 format. Only present if parsed is true.</rdfs:comment>
    <rdfs:domain rdf:resource="http://example.org/onto/class/google_kms_ekm_connection"/>
    <rdfs:range rdf:resource="http://www.w3.org/2001/XMLSchema#string"/>
  </owl:DatatypeProperty>
  <owl:DatatypeProperty rdf:about="http://example.org/onto/prop/google_kms_ekm_connection_not_after_time">
    <rdfs:label>not_after_time</rdfs:label>
    <rdfs:comment>Output only. The certificate is not valid after this time. Only present if parsed is true.
A timestamp in RFC3339 UTC "Zulu" format, with nanosecond resolution and up to nine fractional digits. Examples: "2014-10-02T15:01:23Z" and "2014-10-02T15:01:23.045123456Z".</rdfs:comment>
    <rdfs:domain rdf:resource="http://example.org/onto/class/google_kms_ekm_connection"/>
    <rdfs:range rdf:resource="http://www.w3.org/2001/XMLSchema#string"/>
  </owl:DatatypeProperty>
  <owl:DatatypeProperty rdf:about="http://example.org/onto/prop/google_kms_ekm_connection_not_before_time">
    <rdfs:label>not_before_time</rdfs:label>
    <rdfs:comment>Output only. The certificate is not valid before this time. Only present if parsed is true.
A timestamp in RFC3339 UTC "Zulu" format, with nanosecond resolution and up to nine fractional digits. Examples: "2014-10-02T15:01:23Z" and "2014-10-02T15:01:23.045123456Z".</rdfs:comment>
    <rdfs:domain rdf:resource="http://example.org/onto/class/google_kms_ekm_connection"/>
    <rdfs:range rdf:resource="http://www.w3.org/2001/XMLSchema#string"/>
  </owl:DatatypeProperty>
  <owl:DatatypeProperty rdf:about="http://example.org/onto/prop/google_kms_ekm_connection_parsed">
    <rdfs:label>parsed</rdfs:label>
    <rdfs:comment>Output only. True if the certificate was parsed successfully.</rdfs:comment>
    <rdfs:domain rdf:resource="http://example.org/onto/class/google_kms_ekm_connection"/>
    <rdfs:range rdf:resource="http://www.w3.org/2001/XMLSchema#string"/>
  </owl:DatatypeProperty>
  <owl:DatatypeProperty rdf:about="http://example.org/onto/prop/google_kms_ekm_connection_raw_der">
    <rdfs:label>raw_der</rdfs:label>
    <rdfs:comment>Required. The raw certificate bytes in DER format. A base64-encoded string.</rdfs:comment>
    <rdfs:domain rdf:resource="http://example.org/onto/class/google_kms_ekm_connection"/>
    <rdfs:range rdf:resource="http://www.w3.org/2001/XMLSchema#string"/>
  </owl:DatatypeProperty>
  <owl:DatatypeProperty rdf:about="http://example.org/onto/prop/google_kms_ekm_connection_serial_number">
    <rdfs:label>serial_number</rdfs:label>
    <rdfs:comment>Output only. The certificate serial number as a hex string. Only present if parsed is true.</rdfs:comment>
    <rdfs:domain rdf:resource="http://example.org/onto/class/google_kms_ekm_connection"/>
    <rdfs:range rdf:resource="http://www.w3.org/2001/XMLSchema#string"/>
  </owl:DatatypeProperty>
  <owl:DatatypeProperty rdf:about="http://example.org/onto/prop/google_kms_ekm_connection_sha256_fingerprint">
    <rdfs:label>sha256_fingerprint</rdfs:label>
    <rdfs:comment>Output only. The SHA-256 certificate fingerprint as a hex string. Only present if parsed is true.</rdfs:comment>
    <rdfs:domain rdf:resource="http://example.org/onto/class/google_kms_ekm_connection"/>
    <rdfs:range rdf:resource="http://www.w3.org/2001/XMLSchema#string"/>
  </owl:DatatypeProperty>
  <owl:DatatypeProperty rdf:about="http://example.org/onto/prop/google_kms_ekm_connection_subject">
    <rdfs:label>subject</rdfs:label>
    <rdfs:comment>Output only. The subject distinguished name in RFC 2253 format. Only present if parsed is true.</rdfs:comment>
    <rdfs:domain rdf:resource="http://example.org/onto/class/google_kms_ekm_connection"/>
    <rdfs:range rdf:resource="http://www.w3.org/2001/XMLSchema#string"/>
  </owl:DatatypeProperty>
  <owl:DatatypeProperty rdf:about="http://example.org/onto/prop/google_kms_ekm_connection_subject_alternative_dns_names">
    <rdfs:label>subject_alternative_dns_names</rdfs:label>
    <rdfs:comment>Output only. The subject Alternative DNS names. Only present if parsed is true.</rdfs:comment>
    <rdfs:domain rdf:resource="http://example.org/onto/class/google_kms_ekm_connection"/>
    <rdfs:range rdf:resource="http://www.w3.org/2001/XMLSchema#string"/>
  </owl:DatatypeProperty>
  <owl:DatatypeProperty rdf:about="http://example.org/onto/prop/google_kms_ekm_connection_create">
    <rdfs:label>create</rdfs:label>
    <rdfs:domain rdf:resource="http://example.org/onto/class/google_kms_ekm_connection"/>
    <rdfs:range rdf:resource="http://www.w3.org/2001/XMLSchema#string"/>
  </owl:DatatypeProperty>
  <owl:DatatypeProperty rdf:about="http://example.org/onto/prop/google_kms_ekm_connection_delete">
    <rdfs:label>delete</rdfs:label>
    <rdfs:domain rdf:resource="http://example.org/onto/class/google_kms_ekm_connection"/>
    <rdfs:range rdf:resource="http://www.w3.org/2001/XMLSchema#string"/>
  </owl:DatatypeProperty>
  <owl:DatatypeProperty rdf:about="http://example.org/onto/prop/google_kms_ekm_connection_update">
    <rdfs:label>update</rdfs:label>
    <rdfs:domain rdf:resource="http://example.org/onto/class/google_kms_ekm_connection"/>
    <rdfs:range rdf:resource="http://www.w3.org/2001/XMLSchema#string"/>
  </owl:DatatypeProperty>
</rdf:RDF>
