<?xml version="1.0" encoding="UTF-8"?>
<rdf:RDF
  xmlns:rdf="http://www.w3.org/1999/02/22-rdf-syntax-ns#"
  xmlns:rdfs="http://www.w3.org/2000/01/rdf-schema#"
  xmlns:owl="http://www.w3.org/2002/07/owl#"
  xmlns:xsd="http://www.w3.org/2001/XMLSchema#"
  xml:base="http://example.org/onto/">
  <owl:Class rdf:about="http://example.org/onto/class/google_spanner_instance_config">
    <rdfs:label>google_spanner_instance_config</rdfs:label>
    <rdfs:comment>#
#     ***     AUTO GENERATED CODE    ***    Type: MMv1     ***
#
# ----------------------------------------------------------------------------
#
#     This code is generated by Magic Modules using the following:
#
#     Configuration: https:#github.com/GoogleCloudPlatform/magic-modules/tree/main/mmv1/products/spanner/InstanceConfig.yaml
#     Template:      https:#github.com/GoogleCloudPlatform/magic-modules/tree/main/mmv1/templates/terraform/resource.html.markdown.tmpl
#
#     DO NOT EDIT this file directly. Any changes made to this file will be
#     overwritten during the next generation cycle.
#
# ----------------------------------------------------------------------------
subcategory: "Cloud Spanner"
description: |-
  A possible configuration for a Cloud Spanner instance.
---</rdfs:comment>
  </owl:Class>
  <owl:DatatypeProperty rdf:about="http://example.org/onto/prop/google_spanner_instance_config_base_config">
    <rdfs:label>base_config</rdfs:label>
    <rdfs:comment>Base configuration name, e.g. nam3, based on which this configuration is created.
Only set for user managed configurations.
baseConfig must refer to a configuration of type GOOGLE_MANAGED in the same project as this configuration.</rdfs:comment>
    <rdfs:domain rdf:resource="http://example.org/onto/class/google_spanner_instance_config"/>
    <rdfs:range rdf:resource="http://www.w3.org/2001/XMLSchema#string"/>
  </owl:DatatypeProperty>
  <owl:DatatypeProperty rdf:about="http://example.org/onto/prop/google_spanner_instance_config_config_type">
    <rdfs:label>config_type</rdfs:label>
    <rdfs:comment>Output only. Whether this instance config is a Google or User Managed Configuration.</rdfs:comment>
    <rdfs:domain rdf:resource="http://example.org/onto/class/google_spanner_instance_config"/>
    <rdfs:range rdf:resource="http://www.w3.org/2001/XMLSchema#string"/>
  </owl:DatatypeProperty>
  <owl:DatatypeProperty rdf:about="http://example.org/onto/prop/google_spanner_instance_config_display_name">
    <rdfs:label>display_name</rdfs:label>
    <rdfs:comment>The name of this instance configuration as it appears in UIs.</rdfs:comment>
    <rdfs:domain rdf:resource="http://example.org/onto/class/google_spanner_instance_config"/>
    <rdfs:range rdf:resource="http://www.w3.org/2001/XMLSchema#string"/>
  </owl:DatatypeProperty>
  <owl:DatatypeProperty rdf:about="http://example.org/onto/prop/google_spanner_instance_config_effective_labels">
    <rdfs:label>effective_labels</rdfs:label>
    <rdfs:comment>All of labels (key/value pairs) present on the resource in GCP, including the labels configured through Terraform, other clients and services.</rdfs:comment>
    <rdfs:domain rdf:resource="http://example.org/onto/class/google_spanner_instance_config"/>
    <rdfs:range rdf:resource="http://www.w3.org/2001/XMLSchema#string"/>
  </owl:DatatypeProperty>
  <owl:DatatypeProperty rdf:about="http://example.org/onto/prop/google_spanner_instance_config_id">
    <rdfs:label>id</rdfs:label>
    <rdfs:domain rdf:resource="http://example.org/onto/class/google_spanner_instance_config"/>
    <rdfs:range rdf:resource="http://www.w3.org/2001/XMLSchema#string"/>
  </owl:DatatypeProperty>
  <owl:DatatypeProperty rdf:about="http://example.org/onto/prop/google_spanner_instance_config_labels">
    <rdfs:label>labels</rdfs:label>
    <rdfs:comment>An object containing a list of "key": value pairs.
Example: { "name": "wrench", "mass": "1.3kg", "count": "3" }.


**Note**: This field is non-authoritative, and will only manage the labels present in your configuration.
Please refer to the field 'effective_labels' for all of the labels present on the resource.</rdfs:comment>
    <rdfs:domain rdf:resource="http://example.org/onto/class/google_spanner_instance_config"/>
    <rdfs:range rdf:resource="http://www.w3.org/2001/XMLSchema#string"/>
  </owl:DatatypeProperty>
  <owl:DatatypeProperty rdf:about="http://example.org/onto/prop/google_spanner_instance_config_name">
    <rdfs:label>name</rdfs:label>
    <rdfs:comment>A unique identifier for the instance configuration. Values are of the
form projects/<project>/instanceConfigs/[a-z][-a-z0-9]*</rdfs:comment>
    <rdfs:domain rdf:resource="http://example.org/onto/class/google_spanner_instance_config"/>
    <rdfs:range rdf:resource="http://www.w3.org/2001/XMLSchema#string"/>
  </owl:DatatypeProperty>
  <owl:DatatypeProperty rdf:about="http://example.org/onto/prop/google_spanner_instance_config_project">
    <rdfs:label>project</rdfs:label>
    <rdfs:domain rdf:resource="http://example.org/onto/class/google_spanner_instance_config"/>
    <rdfs:range rdf:resource="http://www.w3.org/2001/XMLSchema#string"/>
  </owl:DatatypeProperty>
  <owl:DatatypeProperty rdf:about="http://example.org/onto/prop/google_spanner_instance_config_terraform_labels">
    <rdfs:label>terraform_labels</rdfs:label>
    <rdfs:comment>The combination of labels configured directly on the resource
 and default labels configured on the provider.</rdfs:comment>
    <rdfs:domain rdf:resource="http://example.org/onto/class/google_spanner_instance_config"/>
    <rdfs:range rdf:resource="http://www.w3.org/2001/XMLSchema#string"/>
  </owl:DatatypeProperty>
  <owl:DatatypeProperty rdf:about="http://example.org/onto/prop/google_spanner_instance_config_default_leader_location">
    <rdfs:label>default_leader_location</rdfs:label>
    <rdfs:comment>If true, this location is designated as the default leader location where
leader replicas are placed.</rdfs:comment>
    <rdfs:domain rdf:resource="http://example.org/onto/class/google_spanner_instance_config"/>
    <rdfs:range rdf:resource="http://www.w3.org/2001/XMLSchema#string"/>
  </owl:DatatypeProperty>
  <owl:DatatypeProperty rdf:about="http://example.org/onto/prop/google_spanner_instance_config_location">
    <rdfs:label>location</rdfs:label>
    <rdfs:comment>The location of the serving resources, e.g. "us-central1".</rdfs:comment>
    <rdfs:domain rdf:resource="http://example.org/onto/class/google_spanner_instance_config"/>
    <rdfs:range rdf:resource="http://www.w3.org/2001/XMLSchema#string"/>
  </owl:DatatypeProperty>
  <owl:DatatypeProperty rdf:about="http://example.org/onto/prop/google_spanner_instance_config_type">
    <rdfs:label>type</rdfs:label>
    <rdfs:comment>Indicates the type of replica.  See the [replica types
documentation](https://cloud.google.com/spanner/docs/replication#replica_types)
for more details. Possible values: ["READ_WRITE", "READ_ONLY", "WITNESS"]</rdfs:comment>
    <rdfs:domain rdf:resource="http://example.org/onto/class/google_spanner_instance_config"/>
    <rdfs:range rdf:resource="http://www.w3.org/2001/XMLSchema#string"/>
  </owl:DatatypeProperty>
  <owl:DatatypeProperty rdf:about="http://example.org/onto/prop/google_spanner_instance_config_create">
    <rdfs:label>create</rdfs:label>
    <rdfs:domain rdf:resource="http://example.org/onto/class/google_spanner_instance_config"/>
    <rdfs:range rdf:resource="http://www.w3.org/2001/XMLSchema#string"/>
  </owl:DatatypeProperty>
  <owl:DatatypeProperty rdf:about="http://example.org/onto/prop/google_spanner_instance_config_delete">
    <rdfs:label>delete</rdfs:label>
    <rdfs:domain rdf:resource="http://example.org/onto/class/google_spanner_instance_config"/>
    <rdfs:range rdf:resource="http://www.w3.org/2001/XMLSchema#string"/>
  </owl:DatatypeProperty>
  <owl:DatatypeProperty rdf:about="http://example.org/onto/prop/google_spanner_instance_config_update">
    <rdfs:label>update</rdfs:label>
    <rdfs:domain rdf:resource="http://example.org/onto/class/google_spanner_instance_config"/>
    <rdfs:range rdf:resource="http://www.w3.org/2001/XMLSchema#string"/>
  </owl:DatatypeProperty>
</rdf:RDF>
