<?xml version="1.0" encoding="UTF-8"?>
<rdf:RDF
  xmlns:rdf="http://www.w3.org/1999/02/22-rdf-syntax-ns#"
  xmlns:rdfs="http://www.w3.org/2000/01/rdf-schema#"
  xmlns:owl="http://www.w3.org/2002/07/owl#"
  xmlns:xsd="http://www.w3.org/2001/XMLSchema#"
  xml:base="http://example.org/onto/">
  <owl:Class rdf:about="http://example.org/onto/class/google_bigtable_app_profile">
    <rdfs:label>google_bigtable_app_profile</rdfs:label>
    <rdfs:comment>#
#     ***     AUTO GENERATED CODE    ***    Type: MMv1     ***
#
# ----------------------------------------------------------------------------
#
#     This code is generated by Magic Modules using the following:
#
#     Configuration: https:#github.com/GoogleCloudPlatform/magic-modules/tree/main/mmv1/products/bigtable/AppProfile.yaml
#     Template:      https:#github.com/GoogleCloudPlatform/magic-modules/tree/main/mmv1/templates/terraform/resource.html.markdown.tmpl
#
#     DO NOT EDIT this file directly. Any changes made to this file will be
#     overwritten during the next generation cycle.
#
# ----------------------------------------------------------------------------
subcategory: "Cloud Bigtable"
description: |-
  App profile is a configuration object describing how Cloud Bigtable should treat traffic from a particular end user application.
---</rdfs:comment>
  </owl:Class>
  <owl:DatatypeProperty rdf:about="http://example.org/onto/prop/google_bigtable_app_profile_app_profile_id">
    <rdfs:label>app_profile_id</rdfs:label>
    <rdfs:comment>The unique name of the app profile in the form '[_a-zA-Z0-9][-_.a-zA-Z0-9]*'.</rdfs:comment>
    <rdfs:domain rdf:resource="http://example.org/onto/class/google_bigtable_app_profile"/>
    <rdfs:range rdf:resource="http://www.w3.org/2001/XMLSchema#string"/>
  </owl:DatatypeProperty>
  <owl:DatatypeProperty rdf:about="http://example.org/onto/prop/google_bigtable_app_profile_description">
    <rdfs:label>description</rdfs:label>
    <rdfs:comment>Long form description of the use case for this app profile.</rdfs:comment>
    <rdfs:domain rdf:resource="http://example.org/onto/class/google_bigtable_app_profile"/>
    <rdfs:range rdf:resource="http://www.w3.org/2001/XMLSchema#string"/>
  </owl:DatatypeProperty>
  <owl:DatatypeProperty rdf:about="http://example.org/onto/prop/google_bigtable_app_profile_id">
    <rdfs:label>id</rdfs:label>
    <rdfs:domain rdf:resource="http://example.org/onto/class/google_bigtable_app_profile"/>
    <rdfs:range rdf:resource="http://www.w3.org/2001/XMLSchema#string"/>
  </owl:DatatypeProperty>
  <owl:DatatypeProperty rdf:about="http://example.org/onto/prop/google_bigtable_app_profile_ignore_warnings">
    <rdfs:label>ignore_warnings</rdfs:label>
    <rdfs:comment>If true, ignore safety checks when deleting/updating the app profile.</rdfs:comment>
    <rdfs:domain rdf:resource="http://example.org/onto/class/google_bigtable_app_profile"/>
    <rdfs:range rdf:resource="http://www.w3.org/2001/XMLSchema#string"/>
  </owl:DatatypeProperty>
  <owl:DatatypeProperty rdf:about="http://example.org/onto/prop/google_bigtable_app_profile_instance">
    <rdfs:label>instance</rdfs:label>
    <rdfs:comment>The name of the instance to create the app profile within.</rdfs:comment>
    <rdfs:domain rdf:resource="http://example.org/onto/class/google_bigtable_app_profile"/>
    <rdfs:range rdf:resource="http://www.w3.org/2001/XMLSchema#string"/>
  </owl:DatatypeProperty>
  <owl:DatatypeProperty rdf:about="http://example.org/onto/prop/google_bigtable_app_profile_multi_cluster_routing_cluster_ids">
    <rdfs:label>multi_cluster_routing_cluster_ids</rdfs:label>
    <rdfs:comment>The set of clusters to route to. The order is ignored; clusters will be tried in order of distance. If left empty, all clusters are eligible.</rdfs:comment>
    <rdfs:domain rdf:resource="http://example.org/onto/class/google_bigtable_app_profile"/>
    <rdfs:range rdf:resource="http://www.w3.org/2001/XMLSchema#string"/>
  </owl:DatatypeProperty>
  <owl:DatatypeProperty rdf:about="http://example.org/onto/prop/google_bigtable_app_profile_multi_cluster_routing_use_any">
    <rdfs:label>multi_cluster_routing_use_any</rdfs:label>
    <rdfs:comment>If true, read/write requests are routed to the nearest cluster in the instance, and will fail over to the nearest cluster that is available
in the event of transient errors or delays. Clusters in a region are considered equidistant. Choosing this option sacrifices read-your-writes
consistency to improve availability.</rdfs:comment>
    <rdfs:domain rdf:resource="http://example.org/onto/class/google_bigtable_app_profile"/>
    <rdfs:range rdf:resource="http://www.w3.org/2001/XMLSchema#string"/>
  </owl:DatatypeProperty>
  <owl:DatatypeProperty rdf:about="http://example.org/onto/prop/google_bigtable_app_profile_name">
    <rdfs:label>name</rdfs:label>
    <rdfs:comment>The unique name of the requested app profile. Values are of the form 'projects/<project>/instances/<instance>/appProfiles/<appProfileId>'.</rdfs:comment>
    <rdfs:domain rdf:resource="http://example.org/onto/class/google_bigtable_app_profile"/>
    <rdfs:range rdf:resource="http://www.w3.org/2001/XMLSchema#string"/>
  </owl:DatatypeProperty>
  <owl:DatatypeProperty rdf:about="http://example.org/onto/prop/google_bigtable_app_profile_project">
    <rdfs:label>project</rdfs:label>
    <rdfs:domain rdf:resource="http://example.org/onto/class/google_bigtable_app_profile"/>
    <rdfs:range rdf:resource="http://www.w3.org/2001/XMLSchema#string"/>
  </owl:DatatypeProperty>
  <owl:DatatypeProperty rdf:about="http://example.org/onto/prop/google_bigtable_app_profile_row_affinity">
    <rdfs:label>row_affinity</rdfs:label>
    <rdfs:comment>Must be used with multi-cluster routing. If true, then this app profile will use row affinity sticky routing. With row affinity, Bigtable will route single row key requests based on the row key, rather than randomly. Instead, each row key will be assigned to a cluster by Cloud Bigtable, and will stick to that cluster. Choosing this option improves read-your-writes consistency for most requests under most circumstances, without sacrificing availability. Consistency is not guaranteed, as requests may still fail over between clusters in the event of errors or latency.</rdfs:comment>
    <rdfs:domain rdf:resource="http://example.org/onto/class/google_bigtable_app_profile"/>
    <rdfs:range rdf:resource="http://www.w3.org/2001/XMLSchema#string"/>
  </owl:DatatypeProperty>
  <owl:DatatypeProperty rdf:about="http://example.org/onto/prop/google_bigtable_app_profile_compute_billing_owner">
    <rdfs:label>compute_billing_owner</rdfs:label>
    <rdfs:comment>The Compute Billing Owner for this Data Boost App Profile. Possible values: ["HOST_PAYS"]</rdfs:comment>
    <rdfs:domain rdf:resource="http://example.org/onto/class/google_bigtable_app_profile"/>
    <rdfs:range rdf:resource="http://www.w3.org/2001/XMLSchema#string"/>
  </owl:DatatypeProperty>
  <owl:DatatypeProperty rdf:about="http://example.org/onto/prop/google_bigtable_app_profile_allow_transactional_writes">
    <rdfs:label>allow_transactional_writes</rdfs:label>
    <rdfs:comment>If true, CheckAndMutateRow and ReadModifyWriteRow requests are allowed by this app profile.
It is unsafe to send these requests to the same table/row/column in multiple clusters.</rdfs:comment>
    <rdfs:domain rdf:resource="http://example.org/onto/class/google_bigtable_app_profile"/>
    <rdfs:range rdf:resource="http://www.w3.org/2001/XMLSchema#string"/>
  </owl:DatatypeProperty>
  <owl:DatatypeProperty rdf:about="http://example.org/onto/prop/google_bigtable_app_profile_cluster_id">
    <rdfs:label>cluster_id</rdfs:label>
    <rdfs:comment>The cluster to which read/write requests should be routed.</rdfs:comment>
    <rdfs:domain rdf:resource="http://example.org/onto/class/google_bigtable_app_profile"/>
    <rdfs:range rdf:resource="http://www.w3.org/2001/XMLSchema#string"/>
  </owl:DatatypeProperty>
  <owl:DatatypeProperty rdf:about="http://example.org/onto/prop/google_bigtable_app_profile_priority">
    <rdfs:label>priority</rdfs:label>
    <rdfs:comment>The priority of requests sent using this app profile. Possible values: ["PRIORITY_LOW", "PRIORITY_MEDIUM", "PRIORITY_HIGH"]</rdfs:comment>
    <rdfs:domain rdf:resource="http://example.org/onto/class/google_bigtable_app_profile"/>
    <rdfs:range rdf:resource="http://www.w3.org/2001/XMLSchema#string"/>
  </owl:DatatypeProperty>
  <owl:DatatypeProperty rdf:about="http://example.org/onto/prop/google_bigtable_app_profile_create">
    <rdfs:label>create</rdfs:label>
    <rdfs:domain rdf:resource="http://example.org/onto/class/google_bigtable_app_profile"/>
    <rdfs:range rdf:resource="http://www.w3.org/2001/XMLSchema#string"/>
  </owl:DatatypeProperty>
  <owl:DatatypeProperty rdf:about="http://example.org/onto/prop/google_bigtable_app_profile_delete">
    <rdfs:label>delete</rdfs:label>
    <rdfs:domain rdf:resource="http://example.org/onto/class/google_bigtable_app_profile"/>
    <rdfs:range rdf:resource="http://www.w3.org/2001/XMLSchema#string"/>
  </owl:DatatypeProperty>
  <owl:DatatypeProperty rdf:about="http://example.org/onto/prop/google_bigtable_app_profile_update">
    <rdfs:label>update</rdfs:label>
    <rdfs:domain rdf:resource="http://example.org/onto/class/google_bigtable_app_profile"/>
    <rdfs:range rdf:resource="http://www.w3.org/2001/XMLSchema#string"/>
  </owl:DatatypeProperty>
</rdf:RDF>
