<?xml version="1.0" encoding="UTF-8"?>
<rdf:RDF
  xmlns:rdf="http://www.w3.org/1999/02/22-rdf-syntax-ns#"
  xmlns:rdfs="http://www.w3.org/2000/01/rdf-schema#"
  xmlns:owl="http://www.w3.org/2002/07/owl#"
  xmlns:xsd="http://www.w3.org/2001/XMLSchema#"
  xml:base="http://example.org/onto/">
  <owl:Class rdf:about="http://example.org/onto/class/google_network_security_server_tls_policy">
    <rdfs:label>google_network_security_server_tls_policy</rdfs:label>
    <rdfs:comment>#
#     ***     AUTO GENERATED CODE    ***    Type: MMv1     ***
#
# ----------------------------------------------------------------------------
#
#     This code is generated by Magic Modules using the following:
#
#     Configuration: https:#github.com/GoogleCloudPlatform/magic-modules/tree/main/mmv1/products/networksecurity/ServerTlsPolicy.yaml
#     Template:      https:#github.com/GoogleCloudPlatform/magic-modules/tree/main/mmv1/templates/terraform/resource.html.markdown.tmpl
#
#     DO NOT EDIT this file directly. Any changes made to this file will be
#     overwritten during the next generation cycle.
#
# ----------------------------------------------------------------------------
subcategory: "Network Security"
description: |-
  ServerTlsPolicy is a resource that specifies how a server should authenticate incoming requests.
---</rdfs:comment>
  </owl:Class>
  <owl:DatatypeProperty rdf:about="http://example.org/onto/prop/google_network_security_server_tls_policy_allow_open">
    <rdfs:label>allow_open</rdfs:label>
    <rdfs:comment>This field applies only for Traffic Director policies. It is must be set to false for external HTTPS load balancer policies.
Determines if server allows plaintext connections. If set to true, server allows plain text connections. By default, it is set to false. This setting is not exclusive of other encryption modes. For example, if allowOpen and mtlsPolicy are set, server allows both plain text and mTLS connections. See documentation of other encryption modes to confirm compatibility.
Consider using it if you wish to upgrade in place your deployment to TLS while having mixed TLS and non-TLS traffic reaching port :80.</rdfs:comment>
    <rdfs:domain rdf:resource="http://example.org/onto/class/google_network_security_server_tls_policy"/>
    <rdfs:range rdf:resource="http://www.w3.org/2001/XMLSchema#string"/>
  </owl:DatatypeProperty>
  <owl:DatatypeProperty rdf:about="http://example.org/onto/prop/google_network_security_server_tls_policy_create_time">
    <rdfs:label>create_time</rdfs:label>
    <rdfs:comment>Time the ServerTlsPolicy was created in UTC.</rdfs:comment>
    <rdfs:domain rdf:resource="http://example.org/onto/class/google_network_security_server_tls_policy"/>
    <rdfs:range rdf:resource="http://www.w3.org/2001/XMLSchema#string"/>
  </owl:DatatypeProperty>
  <owl:DatatypeProperty rdf:about="http://example.org/onto/prop/google_network_security_server_tls_policy_description">
    <rdfs:label>description</rdfs:label>
    <rdfs:comment>A free-text description of the resource. Max length 1024 characters.</rdfs:comment>
    <rdfs:domain rdf:resource="http://example.org/onto/class/google_network_security_server_tls_policy"/>
    <rdfs:range rdf:resource="http://www.w3.org/2001/XMLSchema#string"/>
  </owl:DatatypeProperty>
  <owl:DatatypeProperty rdf:about="http://example.org/onto/prop/google_network_security_server_tls_policy_effective_labels">
    <rdfs:label>effective_labels</rdfs:label>
    <rdfs:comment>All of labels (key/value pairs) present on the resource in GCP, including the labels configured through Terraform, other clients and services.</rdfs:comment>
    <rdfs:domain rdf:resource="http://example.org/onto/class/google_network_security_server_tls_policy"/>
    <rdfs:range rdf:resource="http://www.w3.org/2001/XMLSchema#string"/>
  </owl:DatatypeProperty>
  <owl:DatatypeProperty rdf:about="http://example.org/onto/prop/google_network_security_server_tls_policy_id">
    <rdfs:label>id</rdfs:label>
    <rdfs:domain rdf:resource="http://example.org/onto/class/google_network_security_server_tls_policy"/>
    <rdfs:range rdf:resource="http://www.w3.org/2001/XMLSchema#string"/>
  </owl:DatatypeProperty>
  <owl:DatatypeProperty rdf:about="http://example.org/onto/prop/google_network_security_server_tls_policy_labels">
    <rdfs:label>labels</rdfs:label>
    <rdfs:comment>Set of label tags associated with the ServerTlsPolicy resource.

**Note**: This field is non-authoritative, and will only manage the labels present in your configuration.
Please refer to the field 'effective_labels' for all of the labels present on the resource.</rdfs:comment>
    <rdfs:domain rdf:resource="http://example.org/onto/class/google_network_security_server_tls_policy"/>
    <rdfs:range rdf:resource="http://www.w3.org/2001/XMLSchema#string"/>
  </owl:DatatypeProperty>
  <owl:DatatypeProperty rdf:about="http://example.org/onto/prop/google_network_security_server_tls_policy_location">
    <rdfs:label>location</rdfs:label>
    <rdfs:comment>The location of the server tls policy.
The default value is 'global'.</rdfs:comment>
    <rdfs:domain rdf:resource="http://example.org/onto/class/google_network_security_server_tls_policy"/>
    <rdfs:range rdf:resource="http://www.w3.org/2001/XMLSchema#string"/>
  </owl:DatatypeProperty>
  <owl:DatatypeProperty rdf:about="http://example.org/onto/prop/google_network_security_server_tls_policy_name">
    <rdfs:label>name</rdfs:label>
    <rdfs:comment>Name of the ServerTlsPolicy resource.</rdfs:comment>
    <rdfs:domain rdf:resource="http://example.org/onto/class/google_network_security_server_tls_policy"/>
    <rdfs:range rdf:resource="http://www.w3.org/2001/XMLSchema#string"/>
  </owl:DatatypeProperty>
  <owl:DatatypeProperty rdf:about="http://example.org/onto/prop/google_network_security_server_tls_policy_project">
    <rdfs:label>project</rdfs:label>
    <rdfs:domain rdf:resource="http://example.org/onto/class/google_network_security_server_tls_policy"/>
    <rdfs:range rdf:resource="http://www.w3.org/2001/XMLSchema#string"/>
  </owl:DatatypeProperty>
  <owl:DatatypeProperty rdf:about="http://example.org/onto/prop/google_network_security_server_tls_policy_terraform_labels">
    <rdfs:label>terraform_labels</rdfs:label>
    <rdfs:comment>The combination of labels configured directly on the resource
 and default labels configured on the provider.</rdfs:comment>
    <rdfs:domain rdf:resource="http://example.org/onto/class/google_network_security_server_tls_policy"/>
    <rdfs:range rdf:resource="http://www.w3.org/2001/XMLSchema#string"/>
  </owl:DatatypeProperty>
  <owl:DatatypeProperty rdf:about="http://example.org/onto/prop/google_network_security_server_tls_policy_update_time">
    <rdfs:label>update_time</rdfs:label>
    <rdfs:comment>Time the ServerTlsPolicy was updated in UTC.</rdfs:comment>
    <rdfs:domain rdf:resource="http://example.org/onto/class/google_network_security_server_tls_policy"/>
    <rdfs:range rdf:resource="http://www.w3.org/2001/XMLSchema#string"/>
  </owl:DatatypeProperty>
  <owl:DatatypeProperty rdf:about="http://example.org/onto/prop/google_network_security_server_tls_policy_client_validation_mode">
    <rdfs:label>client_validation_mode</rdfs:label>
    <rdfs:comment>When the client presents an invalid certificate or no certificate to the load balancer, the clientValidationMode specifies how the client connection is handled.
Required if the policy is to be used with the external HTTPS load balancing. For Traffic Director it must be empty. Possible values: ["CLIENT_VALIDATION_MODE_UNSPECIFIED", "ALLOW_INVALID_OR_MISSING_CLIENT_CERT", "REJECT_INVALID"]</rdfs:comment>
    <rdfs:domain rdf:resource="http://example.org/onto/class/google_network_security_server_tls_policy"/>
    <rdfs:range rdf:resource="http://www.w3.org/2001/XMLSchema#string"/>
  </owl:DatatypeProperty>
  <owl:DatatypeProperty rdf:about="http://example.org/onto/prop/google_network_security_server_tls_policy_client_validation_trust_config">
    <rdfs:label>client_validation_trust_config</rdfs:label>
    <rdfs:comment>Reference to the TrustConfig from certificatemanager.googleapis.com namespace.
If specified, the chain validation will be performed against certificates configured in the given TrustConfig.
Allowed only if the policy is to be used with external HTTPS load balancers.</rdfs:comment>
    <rdfs:domain rdf:resource="http://example.org/onto/class/google_network_security_server_tls_policy"/>
    <rdfs:range rdf:resource="http://www.w3.org/2001/XMLSchema#string"/>
  </owl:DatatypeProperty>
  <owl:DatatypeProperty rdf:about="http://example.org/onto/prop/google_network_security_server_tls_policy_plugin_instance">
    <rdfs:label>plugin_instance</rdfs:label>
    <rdfs:comment>Plugin instance name, used to locate and load CertificateProvider instance configuration. Set to "google_cloud_private_spiffe" to use Certificate Authority Service certificate provider instance.</rdfs:comment>
    <rdfs:domain rdf:resource="http://example.org/onto/class/google_network_security_server_tls_policy"/>
    <rdfs:range rdf:resource="http://www.w3.org/2001/XMLSchema#string"/>
  </owl:DatatypeProperty>
  <owl:DatatypeProperty rdf:about="http://example.org/onto/prop/google_network_security_server_tls_policy_target_uri">
    <rdfs:label>target_uri</rdfs:label>
    <rdfs:comment>The target URI of the gRPC endpoint. Only UDS path is supported, and should start with "unix:".</rdfs:comment>
    <rdfs:domain rdf:resource="http://example.org/onto/class/google_network_security_server_tls_policy"/>
    <rdfs:range rdf:resource="http://www.w3.org/2001/XMLSchema#string"/>
  </owl:DatatypeProperty>
  <owl:DatatypeProperty rdf:about="http://example.org/onto/prop/google_network_security_server_tls_policy_plugin_instance">
    <rdfs:label>plugin_instance</rdfs:label>
    <rdfs:comment>Plugin instance name, used to locate and load CertificateProvider instance configuration. Set to "google_cloud_private_spiffe" to use Certificate Authority Service certificate provider instance.</rdfs:comment>
    <rdfs:domain rdf:resource="http://example.org/onto/class/google_network_security_server_tls_policy"/>
    <rdfs:range rdf:resource="http://www.w3.org/2001/XMLSchema#string"/>
  </owl:DatatypeProperty>
  <owl:DatatypeProperty rdf:about="http://example.org/onto/prop/google_network_security_server_tls_policy_target_uri">
    <rdfs:label>target_uri</rdfs:label>
    <rdfs:comment>The target URI of the gRPC endpoint. Only UDS path is supported, and should start with "unix:".</rdfs:comment>
    <rdfs:domain rdf:resource="http://example.org/onto/class/google_network_security_server_tls_policy"/>
    <rdfs:range rdf:resource="http://www.w3.org/2001/XMLSchema#string"/>
  </owl:DatatypeProperty>
  <owl:DatatypeProperty rdf:about="http://example.org/onto/prop/google_network_security_server_tls_policy_create">
    <rdfs:label>create</rdfs:label>
    <rdfs:domain rdf:resource="http://example.org/onto/class/google_network_security_server_tls_policy"/>
    <rdfs:range rdf:resource="http://www.w3.org/2001/XMLSchema#string"/>
  </owl:DatatypeProperty>
  <owl:DatatypeProperty rdf:about="http://example.org/onto/prop/google_network_security_server_tls_policy_delete">
    <rdfs:label>delete</rdfs:label>
    <rdfs:domain rdf:resource="http://example.org/onto/class/google_network_security_server_tls_policy"/>
    <rdfs:range rdf:resource="http://www.w3.org/2001/XMLSchema#string"/>
  </owl:DatatypeProperty>
  <owl:DatatypeProperty rdf:about="http://example.org/onto/prop/google_network_security_server_tls_policy_update">
    <rdfs:label>update</rdfs:label>
    <rdfs:domain rdf:resource="http://example.org/onto/class/google_network_security_server_tls_policy"/>
    <rdfs:range rdf:resource="http://www.w3.org/2001/XMLSchema#string"/>
  </owl:DatatypeProperty>
</rdf:RDF>
