<?xml version="1.0" encoding="UTF-8"?>
<rdf:RDF
  xmlns:rdf="http://www.w3.org/1999/02/22-rdf-syntax-ns#"
  xmlns:rdfs="http://www.w3.org/2000/01/rdf-schema#"
  xmlns:owl="http://www.w3.org/2002/07/owl#"
  xmlns:xsd="http://www.w3.org/2001/XMLSchema#"
  xml:base="http://example.org/onto/">
  <owl:Class rdf:about="http://example.org/onto/class/google_privateca_certificate_authority">
    <rdfs:label>google_privateca_certificate_authority</rdfs:label>
    <rdfs:comment>#
#     ***     AUTO GENERATED CODE    ***    Type: MMv1     ***
#
# ----------------------------------------------------------------------------
#
#     This code is generated by Magic Modules using the following:
#
#     Configuration: https:#github.com/GoogleCloudPlatform/magic-modules/tree/main/mmv1/products/privateca/CertificateAuthority.yaml
#     Template:      https:#github.com/GoogleCloudPlatform/magic-modules/tree/main/mmv1/templates/terraform/resource.html.markdown.tmpl
#
#     DO NOT EDIT this file directly. Any changes made to this file will be
#     overwritten during the next generation cycle.
#
# ----------------------------------------------------------------------------
subcategory: "Certificate Authority Service"
description: |-
  A CertificateAuthority represents an individual Certificate Authority.
---</rdfs:comment>
  </owl:Class>
  <owl:DatatypeProperty rdf:about="http://example.org/onto/prop/google_privateca_certificate_authority_access_urls">
    <rdfs:label>access_urls</rdfs:label>
    <rdfs:comment>URLs for accessing content published by this CA, such as the CA certificate and CRLs.</rdfs:comment>
    <rdfs:domain rdf:resource="http://example.org/onto/class/google_privateca_certificate_authority"/>
    <rdfs:range rdf:resource="http://www.w3.org/2001/XMLSchema#string"/>
  </owl:DatatypeProperty>
  <owl:DatatypeProperty rdf:about="http://example.org/onto/prop/google_privateca_certificate_authority_certificate_authority_id">
    <rdfs:label>certificate_authority_id</rdfs:label>
    <rdfs:comment>The user provided Resource ID for this Certificate Authority.</rdfs:comment>
    <rdfs:domain rdf:resource="http://example.org/onto/class/google_privateca_certificate_authority"/>
    <rdfs:range rdf:resource="http://www.w3.org/2001/XMLSchema#string"/>
  </owl:DatatypeProperty>
  <owl:DatatypeProperty rdf:about="http://example.org/onto/prop/google_privateca_certificate_authority_create_time">
    <rdfs:label>create_time</rdfs:label>
    <rdfs:comment>The time at which this CertificateAuthority was created.

A timestamp in RFC3339 UTC "Zulu" format, with nanosecond resolution and up to nine
fractional digits. Examples: "2014-10-02T15:01:23Z" and "2014-10-02T15:01:23.045123456Z".</rdfs:comment>
    <rdfs:domain rdf:resource="http://example.org/onto/class/google_privateca_certificate_authority"/>
    <rdfs:range rdf:resource="http://www.w3.org/2001/XMLSchema#string"/>
  </owl:DatatypeProperty>
  <owl:DatatypeProperty rdf:about="http://example.org/onto/prop/google_privateca_certificate_authority_deletion_protection">
    <rdfs:label>deletion_protection</rdfs:label>
    <rdfs:comment>Whether Terraform will be prevented from destroying the CertificateAuthority.
When the field is set to true or unset in Terraform state, a 'terraform apply'
or 'terraform destroy' that would delete the CertificateAuthority will fail.
When the field is set to false, deleting the CertificateAuthority is allowed.</rdfs:comment>
    <rdfs:domain rdf:resource="http://example.org/onto/class/google_privateca_certificate_authority"/>
    <rdfs:range rdf:resource="http://www.w3.org/2001/XMLSchema#string"/>
  </owl:DatatypeProperty>
  <owl:DatatypeProperty rdf:about="http://example.org/onto/prop/google_privateca_certificate_authority_desired_state">
    <rdfs:label>desired_state</rdfs:label>
    <rdfs:comment>Desired state of the CertificateAuthority. Set this field to 'STAGED' to create a 'STAGED' root CA.
Possible values: ENABLED, DISABLED, STAGED.</rdfs:comment>
    <rdfs:domain rdf:resource="http://example.org/onto/class/google_privateca_certificate_authority"/>
    <rdfs:range rdf:resource="http://www.w3.org/2001/XMLSchema#string"/>
  </owl:DatatypeProperty>
  <owl:DatatypeProperty rdf:about="http://example.org/onto/prop/google_privateca_certificate_authority_effective_labels">
    <rdfs:label>effective_labels</rdfs:label>
    <rdfs:comment>All of labels (key/value pairs) present on the resource in GCP, including the labels configured through Terraform, other clients and services.</rdfs:comment>
    <rdfs:domain rdf:resource="http://example.org/onto/class/google_privateca_certificate_authority"/>
    <rdfs:range rdf:resource="http://www.w3.org/2001/XMLSchema#string"/>
  </owl:DatatypeProperty>
  <owl:DatatypeProperty rdf:about="http://example.org/onto/prop/google_privateca_certificate_authority_gcs_bucket">
    <rdfs:label>gcs_bucket</rdfs:label>
    <rdfs:comment>The name of a Cloud Storage bucket where this CertificateAuthority will publish content,
such as the CA certificate and CRLs. This must be a bucket name, without any prefixes
(such as 'gs://') or suffixes (such as '.googleapis.com'). For example, to use a bucket named
my-bucket, you would simply specify 'my-bucket'. If not specified, a managed bucket will be
created.</rdfs:comment>
    <rdfs:domain rdf:resource="http://example.org/onto/class/google_privateca_certificate_authority"/>
    <rdfs:range rdf:resource="http://www.w3.org/2001/XMLSchema#string"/>
  </owl:DatatypeProperty>
  <owl:DatatypeProperty rdf:about="http://example.org/onto/prop/google_privateca_certificate_authority_id">
    <rdfs:label>id</rdfs:label>
    <rdfs:domain rdf:resource="http://example.org/onto/class/google_privateca_certificate_authority"/>
    <rdfs:range rdf:resource="http://www.w3.org/2001/XMLSchema#string"/>
  </owl:DatatypeProperty>
  <owl:DatatypeProperty rdf:about="http://example.org/onto/prop/google_privateca_certificate_authority_ignore_active_certificates_on_deletion">
    <rdfs:label>ignore_active_certificates_on_deletion</rdfs:label>
    <rdfs:comment>This field allows the CA to be deleted even if the CA has active certs. Active certs include both unrevoked and unexpired certs.
Use with care. Defaults to 'false'.</rdfs:comment>
    <rdfs:domain rdf:resource="http://example.org/onto/class/google_privateca_certificate_authority"/>
    <rdfs:range rdf:resource="http://www.w3.org/2001/XMLSchema#string"/>
  </owl:DatatypeProperty>
  <owl:DatatypeProperty rdf:about="http://example.org/onto/prop/google_privateca_certificate_authority_labels">
    <rdfs:label>labels</rdfs:label>
    <rdfs:comment>Labels with user-defined metadata.

An object containing a list of "key": value pairs. Example: { "name": "wrench", "mass":
"1.3kg", "count": "3" }.


**Note**: This field is non-authoritative, and will only manage the labels present in your configuration.
Please refer to the field 'effective_labels' for all of the labels present on the resource.</rdfs:comment>
    <rdfs:domain rdf:resource="http://example.org/onto/class/google_privateca_certificate_authority"/>
    <rdfs:range rdf:resource="http://www.w3.org/2001/XMLSchema#string"/>
  </owl:DatatypeProperty>
  <owl:DatatypeProperty rdf:about="http://example.org/onto/prop/google_privateca_certificate_authority_lifetime">
    <rdfs:label>lifetime</rdfs:label>
    <rdfs:comment>The desired lifetime of the CA certificate. Used to create the "notBeforeTime" and
"notAfterTime" fields inside an X.509 certificate. A duration in seconds with up to nine
fractional digits, terminated by 's'. Example: "3.5s".</rdfs:comment>
    <rdfs:domain rdf:resource="http://example.org/onto/class/google_privateca_certificate_authority"/>
    <rdfs:range rdf:resource="http://www.w3.org/2001/XMLSchema#string"/>
  </owl:DatatypeProperty>
  <owl:DatatypeProperty rdf:about="http://example.org/onto/prop/google_privateca_certificate_authority_location">
    <rdfs:label>location</rdfs:label>
    <rdfs:comment>Location of the CertificateAuthority. A full list of valid locations can be found by
running 'gcloud privateca locations list'.</rdfs:comment>
    <rdfs:domain rdf:resource="http://example.org/onto/class/google_privateca_certificate_authority"/>
    <rdfs:range rdf:resource="http://www.w3.org/2001/XMLSchema#string"/>
  </owl:DatatypeProperty>
  <owl:DatatypeProperty rdf:about="http://example.org/onto/prop/google_privateca_certificate_authority_name">
    <rdfs:label>name</rdfs:label>
    <rdfs:comment>The resource name for this CertificateAuthority in the format
projects/*/locations/*/certificateAuthorities/*.</rdfs:comment>
    <rdfs:domain rdf:resource="http://example.org/onto/class/google_privateca_certificate_authority"/>
    <rdfs:range rdf:resource="http://www.w3.org/2001/XMLSchema#string"/>
  </owl:DatatypeProperty>
  <owl:DatatypeProperty rdf:about="http://example.org/onto/prop/google_privateca_certificate_authority_pem_ca_certificate">
    <rdfs:label>pem_ca_certificate</rdfs:label>
    <rdfs:comment>The signed CA certificate issued from the subordinated CA's CSR. This is needed when activating the subordiante CA with a third party issuer.</rdfs:comment>
    <rdfs:domain rdf:resource="http://example.org/onto/class/google_privateca_certificate_authority"/>
    <rdfs:range rdf:resource="http://www.w3.org/2001/XMLSchema#string"/>
  </owl:DatatypeProperty>
  <owl:DatatypeProperty rdf:about="http://example.org/onto/prop/google_privateca_certificate_authority_pem_ca_certificates">
    <rdfs:label>pem_ca_certificates</rdfs:label>
    <rdfs:comment>This CertificateAuthority's certificate chain, including the current
CertificateAuthority's certificate. Ordered such that the root issuer is the final
element (consistent with RFC 5246). For a self-signed CA, this will only list the current
CertificateAuthority's certificate.</rdfs:comment>
    <rdfs:domain rdf:resource="http://example.org/onto/class/google_privateca_certificate_authority"/>
    <rdfs:range rdf:resource="http://www.w3.org/2001/XMLSchema#string"/>
  </owl:DatatypeProperty>
  <owl:DatatypeProperty rdf:about="http://example.org/onto/prop/google_privateca_certificate_authority_pool">
    <rdfs:label>pool</rdfs:label>
    <rdfs:comment>The name of the CaPool this Certificate Authority belongs to.</rdfs:comment>
    <rdfs:domain rdf:resource="http://example.org/onto/class/google_privateca_certificate_authority"/>
    <rdfs:range rdf:resource="http://www.w3.org/2001/XMLSchema#string"/>
  </owl:DatatypeProperty>
  <owl:DatatypeProperty rdf:about="http://example.org/onto/prop/google_privateca_certificate_authority_project">
    <rdfs:label>project</rdfs:label>
    <rdfs:domain rdf:resource="http://example.org/onto/class/google_privateca_certificate_authority"/>
    <rdfs:range rdf:resource="http://www.w3.org/2001/XMLSchema#string"/>
  </owl:DatatypeProperty>
  <owl:DatatypeProperty rdf:about="http://example.org/onto/prop/google_privateca_certificate_authority_skip_grace_period">
    <rdfs:label>skip_grace_period</rdfs:label>
    <rdfs:comment>If this flag is set, the Certificate Authority will be deleted as soon as
possible without a 30-day grace period where undeletion would have been
allowed. If you proceed, there will be no way to recover this CA.
Use with care. Defaults to 'false'.</rdfs:comment>
    <rdfs:domain rdf:resource="http://example.org/onto/class/google_privateca_certificate_authority"/>
    <rdfs:range rdf:resource="http://www.w3.org/2001/XMLSchema#string"/>
  </owl:DatatypeProperty>
  <owl:DatatypeProperty rdf:about="http://example.org/onto/prop/google_privateca_certificate_authority_state">
    <rdfs:label>state</rdfs:label>
    <rdfs:comment>The State for this CertificateAuthority.</rdfs:comment>
    <rdfs:domain rdf:resource="http://example.org/onto/class/google_privateca_certificate_authority"/>
    <rdfs:range rdf:resource="http://www.w3.org/2001/XMLSchema#string"/>
  </owl:DatatypeProperty>
  <owl:DatatypeProperty rdf:about="http://example.org/onto/prop/google_privateca_certificate_authority_terraform_labels">
    <rdfs:label>terraform_labels</rdfs:label>
    <rdfs:comment>The combination of labels configured directly on the resource
 and default labels configured on the provider.</rdfs:comment>
    <rdfs:domain rdf:resource="http://example.org/onto/class/google_privateca_certificate_authority"/>
    <rdfs:range rdf:resource="http://www.w3.org/2001/XMLSchema#string"/>
  </owl:DatatypeProperty>
  <owl:DatatypeProperty rdf:about="http://example.org/onto/prop/google_privateca_certificate_authority_type">
    <rdfs:label>type</rdfs:label>
    <rdfs:comment>The Type of this CertificateAuthority.

~> **Note:** For 'SUBORDINATE' Certificate Authorities, they need to
be activated before they can issue certificates. Default value: "SELF_SIGNED" Possible values: ["SELF_SIGNED", "SUBORDINATE"]</rdfs:comment>
    <rdfs:domain rdf:resource="http://example.org/onto/class/google_privateca_certificate_authority"/>
    <rdfs:range rdf:resource="http://www.w3.org/2001/XMLSchema#string"/>
  </owl:DatatypeProperty>
  <owl:DatatypeProperty rdf:about="http://example.org/onto/prop/google_privateca_certificate_authority_update_time">
    <rdfs:label>update_time</rdfs:label>
    <rdfs:comment>The time at which this CertificateAuthority was updated.

A timestamp in RFC3339 UTC "Zulu" format, with nanosecond resolution and up to nine
fractional digits. Examples: "2014-10-02T15:01:23Z" and "2014-10-02T15:01:23.045123456Z".</rdfs:comment>
    <rdfs:domain rdf:resource="http://example.org/onto/class/google_privateca_certificate_authority"/>
    <rdfs:range rdf:resource="http://www.w3.org/2001/XMLSchema#string"/>
  </owl:DatatypeProperty>
  <owl:DatatypeProperty rdf:about="http://example.org/onto/prop/google_privateca_certificate_authority_common_name">
    <rdfs:label>common_name</rdfs:label>
    <rdfs:comment>The common name of the distinguished name.</rdfs:comment>
    <rdfs:domain rdf:resource="http://example.org/onto/class/google_privateca_certificate_authority"/>
    <rdfs:range rdf:resource="http://www.w3.org/2001/XMLSchema#string"/>
  </owl:DatatypeProperty>
  <owl:DatatypeProperty rdf:about="http://example.org/onto/prop/google_privateca_certificate_authority_country_code">
    <rdfs:label>country_code</rdfs:label>
    <rdfs:comment>The country code of the subject.</rdfs:comment>
    <rdfs:domain rdf:resource="http://example.org/onto/class/google_privateca_certificate_authority"/>
    <rdfs:range rdf:resource="http://www.w3.org/2001/XMLSchema#string"/>
  </owl:DatatypeProperty>
  <owl:DatatypeProperty rdf:about="http://example.org/onto/prop/google_privateca_certificate_authority_locality">
    <rdfs:label>locality</rdfs:label>
    <rdfs:comment>The locality or city of the subject.</rdfs:comment>
    <rdfs:domain rdf:resource="http://example.org/onto/class/google_privateca_certificate_authority"/>
    <rdfs:range rdf:resource="http://www.w3.org/2001/XMLSchema#string"/>
  </owl:DatatypeProperty>
  <owl:DatatypeProperty rdf:about="http://example.org/onto/prop/google_privateca_certificate_authority_organization">
    <rdfs:label>organization</rdfs:label>
    <rdfs:comment>The organization of the subject.</rdfs:comment>
    <rdfs:domain rdf:resource="http://example.org/onto/class/google_privateca_certificate_authority"/>
    <rdfs:range rdf:resource="http://www.w3.org/2001/XMLSchema#string"/>
  </owl:DatatypeProperty>
  <owl:DatatypeProperty rdf:about="http://example.org/onto/prop/google_privateca_certificate_authority_organizational_unit">
    <rdfs:label>organizational_unit</rdfs:label>
    <rdfs:comment>The organizational unit of the subject.</rdfs:comment>
    <rdfs:domain rdf:resource="http://example.org/onto/class/google_privateca_certificate_authority"/>
    <rdfs:range rdf:resource="http://www.w3.org/2001/XMLSchema#string"/>
  </owl:DatatypeProperty>
  <owl:DatatypeProperty rdf:about="http://example.org/onto/prop/google_privateca_certificate_authority_postal_code">
    <rdfs:label>postal_code</rdfs:label>
    <rdfs:comment>The postal code of the subject.</rdfs:comment>
    <rdfs:domain rdf:resource="http://example.org/onto/class/google_privateca_certificate_authority"/>
    <rdfs:range rdf:resource="http://www.w3.org/2001/XMLSchema#string"/>
  </owl:DatatypeProperty>
  <owl:DatatypeProperty rdf:about="http://example.org/onto/prop/google_privateca_certificate_authority_province">
    <rdfs:label>province</rdfs:label>
    <rdfs:comment>The province, territory, or regional state of the subject.</rdfs:comment>
    <rdfs:domain rdf:resource="http://example.org/onto/class/google_privateca_certificate_authority"/>
    <rdfs:range rdf:resource="http://www.w3.org/2001/XMLSchema#string"/>
  </owl:DatatypeProperty>
  <owl:DatatypeProperty rdf:about="http://example.org/onto/prop/google_privateca_certificate_authority_street_address">
    <rdfs:label>street_address</rdfs:label>
    <rdfs:comment>The street address of the subject.</rdfs:comment>
    <rdfs:domain rdf:resource="http://example.org/onto/class/google_privateca_certificate_authority"/>
    <rdfs:range rdf:resource="http://www.w3.org/2001/XMLSchema#string"/>
  </owl:DatatypeProperty>
  <owl:DatatypeProperty rdf:about="http://example.org/onto/prop/google_privateca_certificate_authority_dns_names">
    <rdfs:label>dns_names</rdfs:label>
    <rdfs:comment>Contains only valid, fully-qualified host names.</rdfs:comment>
    <rdfs:domain rdf:resource="http://example.org/onto/class/google_privateca_certificate_authority"/>
    <rdfs:range rdf:resource="http://www.w3.org/2001/XMLSchema#string"/>
  </owl:DatatypeProperty>
  <owl:DatatypeProperty rdf:about="http://example.org/onto/prop/google_privateca_certificate_authority_email_addresses">
    <rdfs:label>email_addresses</rdfs:label>
    <rdfs:comment>Contains only valid RFC 2822 E-mail addresses.</rdfs:comment>
    <rdfs:domain rdf:resource="http://example.org/onto/class/google_privateca_certificate_authority"/>
    <rdfs:range rdf:resource="http://www.w3.org/2001/XMLSchema#string"/>
  </owl:DatatypeProperty>
  <owl:DatatypeProperty rdf:about="http://example.org/onto/prop/google_privateca_certificate_authority_ip_addresses">
    <rdfs:label>ip_addresses</rdfs:label>
    <rdfs:comment>Contains only valid 32-bit IPv4 addresses or RFC 4291 IPv6 addresses.</rdfs:comment>
    <rdfs:domain rdf:resource="http://example.org/onto/class/google_privateca_certificate_authority"/>
    <rdfs:range rdf:resource="http://www.w3.org/2001/XMLSchema#string"/>
  </owl:DatatypeProperty>
  <owl:DatatypeProperty rdf:about="http://example.org/onto/prop/google_privateca_certificate_authority_uris">
    <rdfs:label>uris</rdfs:label>
    <rdfs:comment>Contains only valid RFC 3986 URIs.</rdfs:comment>
    <rdfs:domain rdf:resource="http://example.org/onto/class/google_privateca_certificate_authority"/>
    <rdfs:range rdf:resource="http://www.w3.org/2001/XMLSchema#string"/>
  </owl:DatatypeProperty>
  <owl:DatatypeProperty rdf:about="http://example.org/onto/prop/google_privateca_certificate_authority_key_id">
    <rdfs:label>key_id</rdfs:label>
    <rdfs:comment>The value of the KeyId in lowercase hexadecimal.</rdfs:comment>
    <rdfs:domain rdf:resource="http://example.org/onto/class/google_privateca_certificate_authority"/>
    <rdfs:range rdf:resource="http://www.w3.org/2001/XMLSchema#string"/>
  </owl:DatatypeProperty>
  <owl:DatatypeProperty rdf:about="http://example.org/onto/prop/google_privateca_certificate_authority_aia_ocsp_servers">
    <rdfs:label>aia_ocsp_servers</rdfs:label>
    <rdfs:comment>Describes Online Certificate Status Protocol (OCSP) endpoint addresses that appear in the
"Authority Information Access" extension in the certificate.</rdfs:comment>
    <rdfs:domain rdf:resource="http://example.org/onto/class/google_privateca_certificate_authority"/>
    <rdfs:range rdf:resource="http://www.w3.org/2001/XMLSchema#string"/>
  </owl:DatatypeProperty>
  <owl:DatatypeProperty rdf:about="http://example.org/onto/prop/google_privateca_certificate_authority_critical">
    <rdfs:label>critical</rdfs:label>
    <rdfs:comment>Indicates whether or not this extension is critical (i.e., if the client does not know how to
handle this extension, the client should consider this to be an error).</rdfs:comment>
    <rdfs:domain rdf:resource="http://example.org/onto/class/google_privateca_certificate_authority"/>
    <rdfs:range rdf:resource="http://www.w3.org/2001/XMLSchema#string"/>
  </owl:DatatypeProperty>
  <owl:DatatypeProperty rdf:about="http://example.org/onto/prop/google_privateca_certificate_authority_value">
    <rdfs:label>value</rdfs:label>
    <rdfs:comment>The value of this X.509 extension. A base64-encoded string.</rdfs:comment>
    <rdfs:domain rdf:resource="http://example.org/onto/class/google_privateca_certificate_authority"/>
    <rdfs:range rdf:resource="http://www.w3.org/2001/XMLSchema#string"/>
  </owl:DatatypeProperty>
  <owl:DatatypeProperty rdf:about="http://example.org/onto/prop/google_privateca_certificate_authority_object_id_path">
    <rdfs:label>object_id_path</rdfs:label>
    <rdfs:comment>An ObjectId specifies an object identifier (OID). These provide context and describe types in ASN.1 messages.</rdfs:comment>
    <rdfs:domain rdf:resource="http://example.org/onto/class/google_privateca_certificate_authority"/>
    <rdfs:range rdf:resource="http://www.w3.org/2001/XMLSchema#string"/>
  </owl:DatatypeProperty>
  <owl:DatatypeProperty rdf:about="http://example.org/onto/prop/google_privateca_certificate_authority_is_ca">
    <rdfs:label>is_ca</rdfs:label>
    <rdfs:comment>When true, the "CA" in Basic Constraints extension will be set to true.</rdfs:comment>
    <rdfs:domain rdf:resource="http://example.org/onto/class/google_privateca_certificate_authority"/>
    <rdfs:range rdf:resource="http://www.w3.org/2001/XMLSchema#string"/>
  </owl:DatatypeProperty>
  <owl:DatatypeProperty rdf:about="http://example.org/onto/prop/google_privateca_certificate_authority_max_issuer_path_length">
    <rdfs:label>max_issuer_path_length</rdfs:label>
    <rdfs:comment>Refers to the "path length constraint" in Basic Constraints extension. For a CA certificate, this value describes the depth of
subordinate CA certificates that are allowed. If this value is less than 0, the request will fail. Setting the value to 0
requires setting 'zero_max_issuer_path_length = true'.</rdfs:comment>
    <rdfs:domain rdf:resource="http://example.org/onto/class/google_privateca_certificate_authority"/>
    <rdfs:range rdf:resource="http://www.w3.org/2001/XMLSchema#string"/>
  </owl:DatatypeProperty>
  <owl:DatatypeProperty rdf:about="http://example.org/onto/prop/google_privateca_certificate_authority_non_ca">
    <rdfs:label>non_ca</rdfs:label>
    <rdfs:comment>When true, the "CA" in Basic Constraints extension will be set to false.
If both 'is_ca' and 'non_ca' are unset, the extension will be omitted from the CA certificate.</rdfs:comment>
    <rdfs:domain rdf:resource="http://example.org/onto/class/google_privateca_certificate_authority"/>
    <rdfs:range rdf:resource="http://www.w3.org/2001/XMLSchema#string"/>
  </owl:DatatypeProperty>
  <owl:DatatypeProperty rdf:about="http://example.org/onto/prop/google_privateca_certificate_authority_zero_max_issuer_path_length">
    <rdfs:label>zero_max_issuer_path_length</rdfs:label>
    <rdfs:comment>When true, the "path length constraint" in Basic Constraints extension will be set to 0.
If both 'max_issuer_path_length' and 'zero_max_issuer_path_length' are unset,
the max path length will be omitted from the CA certificate.</rdfs:comment>
    <rdfs:domain rdf:resource="http://example.org/onto/class/google_privateca_certificate_authority"/>
    <rdfs:range rdf:resource="http://www.w3.org/2001/XMLSchema#string"/>
  </owl:DatatypeProperty>
  <owl:DatatypeProperty rdf:about="http://example.org/onto/prop/google_privateca_certificate_authority_cert_sign">
    <rdfs:label>cert_sign</rdfs:label>
    <rdfs:comment>The key may be used to sign certificates.</rdfs:comment>
    <rdfs:domain rdf:resource="http://example.org/onto/class/google_privateca_certificate_authority"/>
    <rdfs:range rdf:resource="http://www.w3.org/2001/XMLSchema#string"/>
  </owl:DatatypeProperty>
  <owl:DatatypeProperty rdf:about="http://example.org/onto/prop/google_privateca_certificate_authority_content_commitment">
    <rdfs:label>content_commitment</rdfs:label>
    <rdfs:comment>The key may be used for cryptographic commitments. Note that this may also be referred to as "non-repudiation".</rdfs:comment>
    <rdfs:domain rdf:resource="http://example.org/onto/class/google_privateca_certificate_authority"/>
    <rdfs:range rdf:resource="http://www.w3.org/2001/XMLSchema#string"/>
  </owl:DatatypeProperty>
  <owl:DatatypeProperty rdf:about="http://example.org/onto/prop/google_privateca_certificate_authority_crl_sign">
    <rdfs:label>crl_sign</rdfs:label>
    <rdfs:comment>The key may be used sign certificate revocation lists.</rdfs:comment>
    <rdfs:domain rdf:resource="http://example.org/onto/class/google_privateca_certificate_authority"/>
    <rdfs:range rdf:resource="http://www.w3.org/2001/XMLSchema#string"/>
  </owl:DatatypeProperty>
  <owl:DatatypeProperty rdf:about="http://example.org/onto/prop/google_privateca_certificate_authority_data_encipherment">
    <rdfs:label>data_encipherment</rdfs:label>
    <rdfs:comment>The key may be used to encipher data.</rdfs:comment>
    <rdfs:domain rdf:resource="http://example.org/onto/class/google_privateca_certificate_authority"/>
    <rdfs:range rdf:resource="http://www.w3.org/2001/XMLSchema#string"/>
  </owl:DatatypeProperty>
  <owl:DatatypeProperty rdf:about="http://example.org/onto/prop/google_privateca_certificate_authority_decipher_only">
    <rdfs:label>decipher_only</rdfs:label>
    <rdfs:comment>The key may be used to decipher only.</rdfs:comment>
    <rdfs:domain rdf:resource="http://example.org/onto/class/google_privateca_certificate_authority"/>
    <rdfs:range rdf:resource="http://www.w3.org/2001/XMLSchema#string"/>
  </owl:DatatypeProperty>
  <owl:DatatypeProperty rdf:about="http://example.org/onto/prop/google_privateca_certificate_authority_digital_signature">
    <rdfs:label>digital_signature</rdfs:label>
    <rdfs:comment>The key may be used for digital signatures.</rdfs:comment>
    <rdfs:domain rdf:resource="http://example.org/onto/class/google_privateca_certificate_authority"/>
    <rdfs:range rdf:resource="http://www.w3.org/2001/XMLSchema#string"/>
  </owl:DatatypeProperty>
  <owl:DatatypeProperty rdf:about="http://example.org/onto/prop/google_privateca_certificate_authority_encipher_only">
    <rdfs:label>encipher_only</rdfs:label>
    <rdfs:comment>The key may be used to encipher only.</rdfs:comment>
    <rdfs:domain rdf:resource="http://example.org/onto/class/google_privateca_certificate_authority"/>
    <rdfs:range rdf:resource="http://www.w3.org/2001/XMLSchema#string"/>
  </owl:DatatypeProperty>
  <owl:DatatypeProperty rdf:about="http://example.org/onto/prop/google_privateca_certificate_authority_key_agreement">
    <rdfs:label>key_agreement</rdfs:label>
    <rdfs:comment>The key may be used in a key agreement protocol.</rdfs:comment>
    <rdfs:domain rdf:resource="http://example.org/onto/class/google_privateca_certificate_authority"/>
    <rdfs:range rdf:resource="http://www.w3.org/2001/XMLSchema#string"/>
  </owl:DatatypeProperty>
  <owl:DatatypeProperty rdf:about="http://example.org/onto/prop/google_privateca_certificate_authority_key_encipherment">
    <rdfs:label>key_encipherment</rdfs:label>
    <rdfs:comment>The key may be used to encipher other keys.</rdfs:comment>
    <rdfs:domain rdf:resource="http://example.org/onto/class/google_privateca_certificate_authority"/>
    <rdfs:range rdf:resource="http://www.w3.org/2001/XMLSchema#string"/>
  </owl:DatatypeProperty>
  <owl:DatatypeProperty rdf:about="http://example.org/onto/prop/google_privateca_certificate_authority_client_auth">
    <rdfs:label>client_auth</rdfs:label>
    <rdfs:comment>Corresponds to OID 1.3.6.1.5.5.7.3.2. Officially described as "TLS WWW client authentication", though regularly used for non-WWW TLS.</rdfs:comment>
    <rdfs:domain rdf:resource="http://example.org/onto/class/google_privateca_certificate_authority"/>
    <rdfs:range rdf:resource="http://www.w3.org/2001/XMLSchema#string"/>
  </owl:DatatypeProperty>
  <owl:DatatypeProperty rdf:about="http://example.org/onto/prop/google_privateca_certificate_authority_code_signing">
    <rdfs:label>code_signing</rdfs:label>
    <rdfs:comment>Corresponds to OID 1.3.6.1.5.5.7.3.3. Officially described as "Signing of downloadable executable code client authentication".</rdfs:comment>
    <rdfs:domain rdf:resource="http://example.org/onto/class/google_privateca_certificate_authority"/>
    <rdfs:range rdf:resource="http://www.w3.org/2001/XMLSchema#string"/>
  </owl:DatatypeProperty>
  <owl:DatatypeProperty rdf:about="http://example.org/onto/prop/google_privateca_certificate_authority_email_protection">
    <rdfs:label>email_protection</rdfs:label>
    <rdfs:comment>Corresponds to OID 1.3.6.1.5.5.7.3.4. Officially described as "Email protection".</rdfs:comment>
    <rdfs:domain rdf:resource="http://example.org/onto/class/google_privateca_certificate_authority"/>
    <rdfs:range rdf:resource="http://www.w3.org/2001/XMLSchema#string"/>
  </owl:DatatypeProperty>
  <owl:DatatypeProperty rdf:about="http://example.org/onto/prop/google_privateca_certificate_authority_ocsp_signing">
    <rdfs:label>ocsp_signing</rdfs:label>
    <rdfs:comment>Corresponds to OID 1.3.6.1.5.5.7.3.9. Officially described as "Signing OCSP responses".</rdfs:comment>
    <rdfs:domain rdf:resource="http://example.org/onto/class/google_privateca_certificate_authority"/>
    <rdfs:range rdf:resource="http://www.w3.org/2001/XMLSchema#string"/>
  </owl:DatatypeProperty>
  <owl:DatatypeProperty rdf:about="http://example.org/onto/prop/google_privateca_certificate_authority_server_auth">
    <rdfs:label>server_auth</rdfs:label>
    <rdfs:comment>Corresponds to OID 1.3.6.1.5.5.7.3.1. Officially described as "TLS WWW server authentication", though regularly used for non-WWW TLS.</rdfs:comment>
    <rdfs:domain rdf:resource="http://example.org/onto/class/google_privateca_certificate_authority"/>
    <rdfs:range rdf:resource="http://www.w3.org/2001/XMLSchema#string"/>
  </owl:DatatypeProperty>
  <owl:DatatypeProperty rdf:about="http://example.org/onto/prop/google_privateca_certificate_authority_time_stamping">
    <rdfs:label>time_stamping</rdfs:label>
    <rdfs:comment>Corresponds to OID 1.3.6.1.5.5.7.3.8. Officially described as "Binding the hash of an object to a time".</rdfs:comment>
    <rdfs:domain rdf:resource="http://example.org/onto/class/google_privateca_certificate_authority"/>
    <rdfs:range rdf:resource="http://www.w3.org/2001/XMLSchema#string"/>
  </owl:DatatypeProperty>
  <owl:DatatypeProperty rdf:about="http://example.org/onto/prop/google_privateca_certificate_authority_object_id_path">
    <rdfs:label>object_id_path</rdfs:label>
    <rdfs:comment>An ObjectId specifies an object identifier (OID). These provide context and describe types in ASN.1 messages.</rdfs:comment>
    <rdfs:domain rdf:resource="http://example.org/onto/class/google_privateca_certificate_authority"/>
    <rdfs:range rdf:resource="http://www.w3.org/2001/XMLSchema#string"/>
  </owl:DatatypeProperty>
  <owl:DatatypeProperty rdf:about="http://example.org/onto/prop/google_privateca_certificate_authority_critical">
    <rdfs:label>critical</rdfs:label>
    <rdfs:comment>Indicates whether or not the name constraints are marked critical.</rdfs:comment>
    <rdfs:domain rdf:resource="http://example.org/onto/class/google_privateca_certificate_authority"/>
    <rdfs:range rdf:resource="http://www.w3.org/2001/XMLSchema#string"/>
  </owl:DatatypeProperty>
  <owl:DatatypeProperty rdf:about="http://example.org/onto/prop/google_privateca_certificate_authority_excluded_dns_names">
    <rdfs:label>excluded_dns_names</rdfs:label>
    <rdfs:comment>Contains excluded DNS names. Any DNS name that can be
constructed by simply adding zero or more labels to
the left-hand side of the name satisfies the name constraint.
For example, 'example.com', 'www.example.com', 'www.sub.example.com'
would satisfy 'example.com' while 'example1.com' does not.</rdfs:comment>
    <rdfs:domain rdf:resource="http://example.org/onto/class/google_privateca_certificate_authority"/>
    <rdfs:range rdf:resource="http://www.w3.org/2001/XMLSchema#string"/>
  </owl:DatatypeProperty>
  <owl:DatatypeProperty rdf:about="http://example.org/onto/prop/google_privateca_certificate_authority_excluded_email_addresses">
    <rdfs:label>excluded_email_addresses</rdfs:label>
    <rdfs:comment>Contains the excluded email addresses. The value can be a particular
email address, a hostname to indicate all email addresses on that host or
a domain with a leading period (e.g. '.example.com') to indicate
all email addresses in that domain.</rdfs:comment>
    <rdfs:domain rdf:resource="http://example.org/onto/class/google_privateca_certificate_authority"/>
    <rdfs:range rdf:resource="http://www.w3.org/2001/XMLSchema#string"/>
  </owl:DatatypeProperty>
  <owl:DatatypeProperty rdf:about="http://example.org/onto/prop/google_privateca_certificate_authority_excluded_ip_ranges">
    <rdfs:label>excluded_ip_ranges</rdfs:label>
    <rdfs:comment>Contains the excluded IP ranges. For IPv4 addresses, the ranges
are expressed using CIDR notation as specified in RFC 4632.
For IPv6 addresses, the ranges are expressed in similar encoding as IPv4
addresses.</rdfs:comment>
    <rdfs:domain rdf:resource="http://example.org/onto/class/google_privateca_certificate_authority"/>
    <rdfs:range rdf:resource="http://www.w3.org/2001/XMLSchema#string"/>
  </owl:DatatypeProperty>
  <owl:DatatypeProperty rdf:about="http://example.org/onto/prop/google_privateca_certificate_authority_excluded_uris">
    <rdfs:label>excluded_uris</rdfs:label>
    <rdfs:comment>Contains the excluded URIs that apply to the host part of the name.
The value can be a hostname or a domain with a
leading period (like '.example.com')</rdfs:comment>
    <rdfs:domain rdf:resource="http://example.org/onto/class/google_privateca_certificate_authority"/>
    <rdfs:range rdf:resource="http://www.w3.org/2001/XMLSchema#string"/>
  </owl:DatatypeProperty>
  <owl:DatatypeProperty rdf:about="http://example.org/onto/prop/google_privateca_certificate_authority_permitted_dns_names">
    <rdfs:label>permitted_dns_names</rdfs:label>
    <rdfs:comment>Contains permitted DNS names. Any DNS name that can be
constructed by simply adding zero or more labels to
the left-hand side of the name satisfies the name constraint.
For example, 'example.com', 'www.example.com', 'www.sub.example.com'
would satisfy 'example.com' while 'example1.com' does not.</rdfs:comment>
    <rdfs:domain rdf:resource="http://example.org/onto/class/google_privateca_certificate_authority"/>
    <rdfs:range rdf:resource="http://www.w3.org/2001/XMLSchema#string"/>
  </owl:DatatypeProperty>
  <owl:DatatypeProperty rdf:about="http://example.org/onto/prop/google_privateca_certificate_authority_permitted_email_addresses">
    <rdfs:label>permitted_email_addresses</rdfs:label>
    <rdfs:comment>Contains the permitted email addresses. The value can be a particular
email address, a hostname to indicate all email addresses on that host or
a domain with a leading period (e.g. '.example.com') to indicate
all email addresses in that domain.</rdfs:comment>
    <rdfs:domain rdf:resource="http://example.org/onto/class/google_privateca_certificate_authority"/>
    <rdfs:range rdf:resource="http://www.w3.org/2001/XMLSchema#string"/>
  </owl:DatatypeProperty>
  <owl:DatatypeProperty rdf:about="http://example.org/onto/prop/google_privateca_certificate_authority_permitted_ip_ranges">
    <rdfs:label>permitted_ip_ranges</rdfs:label>
    <rdfs:comment>Contains the permitted IP ranges. For IPv4 addresses, the ranges
are expressed using CIDR notation as specified in RFC 4632.
For IPv6 addresses, the ranges are expressed in similar encoding as IPv4
addresses.</rdfs:comment>
    <rdfs:domain rdf:resource="http://example.org/onto/class/google_privateca_certificate_authority"/>
    <rdfs:range rdf:resource="http://www.w3.org/2001/XMLSchema#string"/>
  </owl:DatatypeProperty>
  <owl:DatatypeProperty rdf:about="http://example.org/onto/prop/google_privateca_certificate_authority_permitted_uris">
    <rdfs:label>permitted_uris</rdfs:label>
    <rdfs:comment>Contains the permitted URIs that apply to the host part of the name.
The value can be a hostname or a domain with a
leading period (like '.example.com')</rdfs:comment>
    <rdfs:domain rdf:resource="http://example.org/onto/class/google_privateca_certificate_authority"/>
    <rdfs:range rdf:resource="http://www.w3.org/2001/XMLSchema#string"/>
  </owl:DatatypeProperty>
  <owl:DatatypeProperty rdf:about="http://example.org/onto/prop/google_privateca_certificate_authority_object_id_path">
    <rdfs:label>object_id_path</rdfs:label>
    <rdfs:comment>An ObjectId specifies an object identifier (OID). These provide context and describe types in ASN.1 messages.</rdfs:comment>
    <rdfs:domain rdf:resource="http://example.org/onto/class/google_privateca_certificate_authority"/>
    <rdfs:range rdf:resource="http://www.w3.org/2001/XMLSchema#string"/>
  </owl:DatatypeProperty>
  <owl:DatatypeProperty rdf:about="http://example.org/onto/prop/google_privateca_certificate_authority_algorithm">
    <rdfs:label>algorithm</rdfs:label>
    <rdfs:comment>The algorithm to use for creating a managed Cloud KMS key for a for a simplified
experience. All managed keys will be have their ProtectionLevel as HSM. Possible values: ["SIGN_HASH_ALGORITHM_UNSPECIFIED", "RSA_PSS_2048_SHA256", "RSA_PSS_3072_SHA256", "RSA_PSS_4096_SHA256", "RSA_PKCS1_2048_SHA256", "RSA_PKCS1_3072_SHA256", "RSA_PKCS1_4096_SHA256", "EC_P256_SHA256", "EC_P384_SHA384"]</rdfs:comment>
    <rdfs:domain rdf:resource="http://example.org/onto/class/google_privateca_certificate_authority"/>
    <rdfs:range rdf:resource="http://www.w3.org/2001/XMLSchema#string"/>
  </owl:DatatypeProperty>
  <owl:DatatypeProperty rdf:about="http://example.org/onto/prop/google_privateca_certificate_authority_cloud_kms_key_version">
    <rdfs:label>cloud_kms_key_version</rdfs:label>
    <rdfs:comment>The resource name for an existing Cloud KMS CryptoKeyVersion in the format
'projects/*/locations/*/keyRings/*/cryptoKeys/*/cryptoKeyVersions/*'.</rdfs:comment>
    <rdfs:domain rdf:resource="http://example.org/onto/class/google_privateca_certificate_authority"/>
    <rdfs:range rdf:resource="http://www.w3.org/2001/XMLSchema#string"/>
  </owl:DatatypeProperty>
  <owl:DatatypeProperty rdf:about="http://example.org/onto/prop/google_privateca_certificate_authority_certificate_authority">
    <rdfs:label>certificate_authority</rdfs:label>
    <rdfs:comment>This can refer to a CertificateAuthority that was used to create a
subordinate CertificateAuthority. This field is used for information
and usability purposes only. The resource name is in the format
'projects/*/locations/*/caPools/*/certificateAuthorities/*'.</rdfs:comment>
    <rdfs:domain rdf:resource="http://example.org/onto/class/google_privateca_certificate_authority"/>
    <rdfs:range rdf:resource="http://www.w3.org/2001/XMLSchema#string"/>
  </owl:DatatypeProperty>
  <owl:DatatypeProperty rdf:about="http://example.org/onto/prop/google_privateca_certificate_authority_pem_certificates">
    <rdfs:label>pem_certificates</rdfs:label>
    <rdfs:comment>Expected to be in leaf-to-root order according to RFC 5246.</rdfs:comment>
    <rdfs:domain rdf:resource="http://example.org/onto/class/google_privateca_certificate_authority"/>
    <rdfs:range rdf:resource="http://www.w3.org/2001/XMLSchema#string"/>
  </owl:DatatypeProperty>
  <owl:DatatypeProperty rdf:about="http://example.org/onto/prop/google_privateca_certificate_authority_create">
    <rdfs:label>create</rdfs:label>
    <rdfs:domain rdf:resource="http://example.org/onto/class/google_privateca_certificate_authority"/>
    <rdfs:range rdf:resource="http://www.w3.org/2001/XMLSchema#string"/>
  </owl:DatatypeProperty>
  <owl:DatatypeProperty rdf:about="http://example.org/onto/prop/google_privateca_certificate_authority_delete">
    <rdfs:label>delete</rdfs:label>
    <rdfs:domain rdf:resource="http://example.org/onto/class/google_privateca_certificate_authority"/>
    <rdfs:range rdf:resource="http://www.w3.org/2001/XMLSchema#string"/>
  </owl:DatatypeProperty>
  <owl:DatatypeProperty rdf:about="http://example.org/onto/prop/google_privateca_certificate_authority_update">
    <rdfs:label>update</rdfs:label>
    <rdfs:domain rdf:resource="http://example.org/onto/class/google_privateca_certificate_authority"/>
    <rdfs:range rdf:resource="http://www.w3.org/2001/XMLSchema#string"/>
  </owl:DatatypeProperty>
  <owl:DatatypeProperty rdf:about="http://example.org/onto/prop/google_privateca_certificate_authority_aia_issuing_certificate_urls">
    <rdfs:label>aia_issuing_certificate_urls</rdfs:label>
    <rdfs:comment>A list of URLs where this CertificateAuthority's CA certificate is published that is specified by users.</rdfs:comment>
    <rdfs:domain rdf:resource="http://example.org/onto/class/google_privateca_certificate_authority"/>
    <rdfs:range rdf:resource="http://www.w3.org/2001/XMLSchema#string"/>
  </owl:DatatypeProperty>
  <owl:DatatypeProperty rdf:about="http://example.org/onto/prop/google_privateca_certificate_authority_crl_access_urls">
    <rdfs:label>crl_access_urls</rdfs:label>
    <rdfs:comment>A list of URLs where this CertificateAuthority's CRLs are published that is specified by users.</rdfs:comment>
    <rdfs:domain rdf:resource="http://example.org/onto/class/google_privateca_certificate_authority"/>
    <rdfs:range rdf:resource="http://www.w3.org/2001/XMLSchema#string"/>
  </owl:DatatypeProperty>
</rdf:RDF>
