<?xml version="1.0" encoding="UTF-8"?>
<rdf:RDF
  xmlns:rdf="http://www.w3.org/1999/02/22-rdf-syntax-ns#"
  xmlns:rdfs="http://www.w3.org/2000/01/rdf-schema#"
  xmlns:owl="http://www.w3.org/2002/07/owl#"
  xmlns:xsd="http://www.w3.org/2001/XMLSchema#"
  xml:base="http://example.org/onto/">
  <owl:Class rdf:about="http://example.org/onto/class/google_sql_ssl_cert">
    <rdfs:label>google_sql_ssl_cert</rdfs:label>
    <rdfs:comment>#
#     ***     AUTO GENERATED CODE    ***    Type: Handwritten     ***
#
# ----------------------------------------------------------------------------
#
#     This code is generated by Magic Modules using the following:
#
#     Source file: https://github.com/GoogleCloudPlatform/magic-modules/tree/main/mmv1/third_party/terraform/website/docs/r/sql_ssl_cert.html.markdown
#
#     DO NOT EDIT this file directly. Any changes made to this file will be
#     overwritten during the next generation cycle.
#
# ----------------------------------------------------------------------------
subcategory: "Cloud SQL"
description: |-
  Creates a new SQL Ssl Cert in Google Cloud SQL.
---</rdfs:comment>
  </owl:Class>
  <owl:DatatypeProperty rdf:about="http://example.org/onto/prop/google_sql_ssl_cert_cert">
    <rdfs:label>cert</rdfs:label>
    <rdfs:comment>The actual certificate data for this client certificate.</rdfs:comment>
    <rdfs:domain rdf:resource="http://example.org/onto/class/google_sql_ssl_cert"/>
    <rdfs:range rdf:resource="http://www.w3.org/2001/XMLSchema#string"/>
  </owl:DatatypeProperty>
  <owl:DatatypeProperty rdf:about="http://example.org/onto/prop/google_sql_ssl_cert_cert_serial_number">
    <rdfs:label>cert_serial_number</rdfs:label>
    <rdfs:comment>The serial number extracted from the certificate data.</rdfs:comment>
    <rdfs:domain rdf:resource="http://example.org/onto/class/google_sql_ssl_cert"/>
    <rdfs:range rdf:resource="http://www.w3.org/2001/XMLSchema#string"/>
  </owl:DatatypeProperty>
  <owl:DatatypeProperty rdf:about="http://example.org/onto/prop/google_sql_ssl_cert_common_name">
    <rdfs:label>common_name</rdfs:label>
    <rdfs:comment>The common name to be used in the certificate to identify the client. Constrained to [a-zA-Z.-_ ]+. Changing this forces a new resource to be created.</rdfs:comment>
    <rdfs:domain rdf:resource="http://example.org/onto/class/google_sql_ssl_cert"/>
    <rdfs:range rdf:resource="http://www.w3.org/2001/XMLSchema#string"/>
  </owl:DatatypeProperty>
  <owl:DatatypeProperty rdf:about="http://example.org/onto/prop/google_sql_ssl_cert_create_time">
    <rdfs:label>create_time</rdfs:label>
    <rdfs:comment>The time when the certificate was created in RFC 3339 format, for example 2012-11-15T16:19:00.094Z.</rdfs:comment>
    <rdfs:domain rdf:resource="http://example.org/onto/class/google_sql_ssl_cert"/>
    <rdfs:range rdf:resource="http://www.w3.org/2001/XMLSchema#string"/>
  </owl:DatatypeProperty>
  <owl:DatatypeProperty rdf:about="http://example.org/onto/prop/google_sql_ssl_cert_expiration_time">
    <rdfs:label>expiration_time</rdfs:label>
    <rdfs:comment>The time when the certificate expires in RFC 3339 format, for example 2012-11-15T16:19:00.094Z.</rdfs:comment>
    <rdfs:domain rdf:resource="http://example.org/onto/class/google_sql_ssl_cert"/>
    <rdfs:range rdf:resource="http://www.w3.org/2001/XMLSchema#string"/>
  </owl:DatatypeProperty>
  <owl:DatatypeProperty rdf:about="http://example.org/onto/prop/google_sql_ssl_cert_id">
    <rdfs:label>id</rdfs:label>
    <rdfs:domain rdf:resource="http://example.org/onto/class/google_sql_ssl_cert"/>
    <rdfs:range rdf:resource="http://www.w3.org/2001/XMLSchema#string"/>
  </owl:DatatypeProperty>
  <owl:DatatypeProperty rdf:about="http://example.org/onto/prop/google_sql_ssl_cert_instance">
    <rdfs:label>instance</rdfs:label>
    <rdfs:comment>The name of the Cloud SQL instance. Changing this forces a new resource to be created.</rdfs:comment>
    <rdfs:domain rdf:resource="http://example.org/onto/class/google_sql_ssl_cert"/>
    <rdfs:range rdf:resource="http://www.w3.org/2001/XMLSchema#string"/>
  </owl:DatatypeProperty>
  <owl:DatatypeProperty rdf:about="http://example.org/onto/prop/google_sql_ssl_cert_private_key">
    <rdfs:label>private_key</rdfs:label>
    <rdfs:comment>The private key associated with the client certificate.</rdfs:comment>
    <rdfs:domain rdf:resource="http://example.org/onto/class/google_sql_ssl_cert"/>
    <rdfs:range rdf:resource="http://www.w3.org/2001/XMLSchema#string"/>
  </owl:DatatypeProperty>
  <owl:DatatypeProperty rdf:about="http://example.org/onto/prop/google_sql_ssl_cert_project">
    <rdfs:label>project</rdfs:label>
    <rdfs:comment>The ID of the project in which the resource belongs. If it is not provided, the provider project is used.</rdfs:comment>
    <rdfs:domain rdf:resource="http://example.org/onto/class/google_sql_ssl_cert"/>
    <rdfs:range rdf:resource="http://www.w3.org/2001/XMLSchema#string"/>
  </owl:DatatypeProperty>
  <owl:DatatypeProperty rdf:about="http://example.org/onto/prop/google_sql_ssl_cert_server_ca_cert">
    <rdfs:label>server_ca_cert</rdfs:label>
    <rdfs:comment>The CA cert of the server this client cert was generated from.</rdfs:comment>
    <rdfs:domain rdf:resource="http://example.org/onto/class/google_sql_ssl_cert"/>
    <rdfs:range rdf:resource="http://www.w3.org/2001/XMLSchema#string"/>
  </owl:DatatypeProperty>
  <owl:DatatypeProperty rdf:about="http://example.org/onto/prop/google_sql_ssl_cert_sha1_fingerprint">
    <rdfs:label>sha1_fingerprint</rdfs:label>
    <rdfs:comment>The SHA1 Fingerprint of the certificate.</rdfs:comment>
    <rdfs:domain rdf:resource="http://example.org/onto/class/google_sql_ssl_cert"/>
    <rdfs:range rdf:resource="http://www.w3.org/2001/XMLSchema#string"/>
  </owl:DatatypeProperty>
  <owl:DatatypeProperty rdf:about="http://example.org/onto/prop/google_sql_ssl_cert_create">
    <rdfs:label>create</rdfs:label>
    <rdfs:domain rdf:resource="http://example.org/onto/class/google_sql_ssl_cert"/>
    <rdfs:range rdf:resource="http://www.w3.org/2001/XMLSchema#string"/>
  </owl:DatatypeProperty>
  <owl:DatatypeProperty rdf:about="http://example.org/onto/prop/google_sql_ssl_cert_delete">
    <rdfs:label>delete</rdfs:label>
    <rdfs:domain rdf:resource="http://example.org/onto/class/google_sql_ssl_cert"/>
    <rdfs:range rdf:resource="http://www.w3.org/2001/XMLSchema#string"/>
  </owl:DatatypeProperty>
</rdf:RDF>
