<?xml version="1.0" encoding="UTF-8"?>
<rdf:RDF
  xmlns:rdf="http://www.w3.org/1999/02/22-rdf-syntax-ns#"
  xmlns:rdfs="http://www.w3.org/2000/01/rdf-schema#"
  xmlns:owl="http://www.w3.org/2002/07/owl#"
  xmlns:xsd="http://www.w3.org/2001/XMLSchema#"
  xml:base="http://example.org/onto/">
  <owl:Class rdf:about="http://example.org/onto/class/google_clouddeploy_automation">
    <rdfs:label>google_clouddeploy_automation</rdfs:label>
    <rdfs:comment>#
#     ***     AUTO GENERATED CODE    ***    Type: MMv1     ***
#
# ----------------------------------------------------------------------------
#
#     This code is generated by Magic Modules using the following:
#
#     Configuration: https:#github.com/GoogleCloudPlatform/magic-modules/tree/main/mmv1/products/clouddeploy/Automation.yaml
#     Template:      https:#github.com/GoogleCloudPlatform/magic-modules/tree/main/mmv1/templates/terraform/resource.html.markdown.tmpl
#
#     DO NOT EDIT this file directly. Any changes made to this file will be
#     overwritten during the next generation cycle.
#
# ----------------------------------------------------------------------------
subcategory: "Cloud Deploy"
description: |-
  An `Automation` enables the automation of manually driven actions for a Delivery Pipeline, which includes Release promotion amongst Targets, Rollout repair and Rollout deployment strategy advancement.
---</rdfs:comment>
  </owl:Class>
  <owl:DatatypeProperty rdf:about="http://example.org/onto/prop/google_clouddeploy_automation_annotations">
    <rdfs:label>annotations</rdfs:label>
    <rdfs:comment>Optional. User annotations. These attributes can only be set and used by the user, and not by Cloud Deploy. Annotations must meet the following constraints: * Annotations are key/value pairs. * Valid annotation keys have two segments: an optional prefix and name, separated by a slash ('/'). * The name segment is required and must be 63 characters or less, beginning and ending with an alphanumeric character ('[a-z0-9A-Z]') with dashes ('-'), underscores ('_'), dots ('.'), and alphanumerics between. * The prefix is optional. If specified, the prefix must be a DNS subdomain: a series of DNS labels separated by dots('.'), not longer than 253 characters in total, followed by a slash ('/'). See https://kubernetes.io/docs/concepts/overview/working-with-objects/annotations/#syntax-and-character-set for more details.

**Note**: This field is non-authoritative, and will only manage the annotations present in your configuration.
Please refer to the field 'effective_annotations' for all of the annotations present on the resource.</rdfs:comment>
    <rdfs:domain rdf:resource="http://example.org/onto/class/google_clouddeploy_automation"/>
    <rdfs:range rdf:resource="http://www.w3.org/2001/XMLSchema#string"/>
  </owl:DatatypeProperty>
  <owl:DatatypeProperty rdf:about="http://example.org/onto/prop/google_clouddeploy_automation_create_time">
    <rdfs:label>create_time</rdfs:label>
    <rdfs:comment>Output only. Time at which the automation was created.</rdfs:comment>
    <rdfs:domain rdf:resource="http://example.org/onto/class/google_clouddeploy_automation"/>
    <rdfs:range rdf:resource="http://www.w3.org/2001/XMLSchema#string"/>
  </owl:DatatypeProperty>
  <owl:DatatypeProperty rdf:about="http://example.org/onto/prop/google_clouddeploy_automation_delivery_pipeline">
    <rdfs:label>delivery_pipeline</rdfs:label>
    <rdfs:comment>The delivery_pipeline for the resource</rdfs:comment>
    <rdfs:domain rdf:resource="http://example.org/onto/class/google_clouddeploy_automation"/>
    <rdfs:range rdf:resource="http://www.w3.org/2001/XMLSchema#string"/>
  </owl:DatatypeProperty>
  <owl:DatatypeProperty rdf:about="http://example.org/onto/prop/google_clouddeploy_automation_description">
    <rdfs:label>description</rdfs:label>
    <rdfs:comment>Optional. Description of the 'Automation'. Max length is 255 characters.</rdfs:comment>
    <rdfs:domain rdf:resource="http://example.org/onto/class/google_clouddeploy_automation"/>
    <rdfs:range rdf:resource="http://www.w3.org/2001/XMLSchema#string"/>
  </owl:DatatypeProperty>
  <owl:DatatypeProperty rdf:about="http://example.org/onto/prop/google_clouddeploy_automation_effective_annotations">
    <rdfs:label>effective_annotations</rdfs:label>
    <rdfs:comment>All of annotations (key/value pairs) present on the resource in GCP, including the annotations configured through Terraform, other clients and services.</rdfs:comment>
    <rdfs:domain rdf:resource="http://example.org/onto/class/google_clouddeploy_automation"/>
    <rdfs:range rdf:resource="http://www.w3.org/2001/XMLSchema#string"/>
  </owl:DatatypeProperty>
  <owl:DatatypeProperty rdf:about="http://example.org/onto/prop/google_clouddeploy_automation_effective_labels">
    <rdfs:label>effective_labels</rdfs:label>
    <rdfs:comment>All of labels (key/value pairs) present on the resource in GCP, including the labels configured through Terraform, other clients and services.</rdfs:comment>
    <rdfs:domain rdf:resource="http://example.org/onto/class/google_clouddeploy_automation"/>
    <rdfs:range rdf:resource="http://www.w3.org/2001/XMLSchema#string"/>
  </owl:DatatypeProperty>
  <owl:DatatypeProperty rdf:about="http://example.org/onto/prop/google_clouddeploy_automation_etag">
    <rdfs:label>etag</rdfs:label>
    <rdfs:comment>Optional. The weak etag of the 'Automation' resource. This checksum is computed by the server based on the value of other fields, and may be sent on update and delete requests to ensure the client has an up-to-date value before proceeding.</rdfs:comment>
    <rdfs:domain rdf:resource="http://example.org/onto/class/google_clouddeploy_automation"/>
    <rdfs:range rdf:resource="http://www.w3.org/2001/XMLSchema#string"/>
  </owl:DatatypeProperty>
  <owl:DatatypeProperty rdf:about="http://example.org/onto/prop/google_clouddeploy_automation_id">
    <rdfs:label>id</rdfs:label>
    <rdfs:domain rdf:resource="http://example.org/onto/class/google_clouddeploy_automation"/>
    <rdfs:range rdf:resource="http://www.w3.org/2001/XMLSchema#string"/>
  </owl:DatatypeProperty>
  <owl:DatatypeProperty rdf:about="http://example.org/onto/prop/google_clouddeploy_automation_labels">
    <rdfs:label>labels</rdfs:label>
    <rdfs:comment>Optional. Labels are attributes that can be set and used by both the user and by Cloud Deploy. Labels must meet the following constraints: * Keys and values can contain only lowercase letters, numeric characters, underscores, and dashes. * All characters must use UTF-8 encoding, and international characters are allowed. * Keys must start with a lowercase letter or international character. * Each resource is limited to a maximum of 64 labels. Both keys and values are additionally constrained to be <= 63 characters.

**Note**: This field is non-authoritative, and will only manage the labels present in your configuration.
Please refer to the field 'effective_labels' for all of the labels present on the resource.</rdfs:comment>
    <rdfs:domain rdf:resource="http://example.org/onto/class/google_clouddeploy_automation"/>
    <rdfs:range rdf:resource="http://www.w3.org/2001/XMLSchema#string"/>
  </owl:DatatypeProperty>
  <owl:DatatypeProperty rdf:about="http://example.org/onto/prop/google_clouddeploy_automation_location">
    <rdfs:label>location</rdfs:label>
    <rdfs:comment>The location for the resource</rdfs:comment>
    <rdfs:domain rdf:resource="http://example.org/onto/class/google_clouddeploy_automation"/>
    <rdfs:range rdf:resource="http://www.w3.org/2001/XMLSchema#string"/>
  </owl:DatatypeProperty>
  <owl:DatatypeProperty rdf:about="http://example.org/onto/prop/google_clouddeploy_automation_name">
    <rdfs:label>name</rdfs:label>
    <rdfs:comment>Name of the 'Automation'.</rdfs:comment>
    <rdfs:domain rdf:resource="http://example.org/onto/class/google_clouddeploy_automation"/>
    <rdfs:range rdf:resource="http://www.w3.org/2001/XMLSchema#string"/>
  </owl:DatatypeProperty>
  <owl:DatatypeProperty rdf:about="http://example.org/onto/prop/google_clouddeploy_automation_project">
    <rdfs:label>project</rdfs:label>
    <rdfs:domain rdf:resource="http://example.org/onto/class/google_clouddeploy_automation"/>
    <rdfs:range rdf:resource="http://www.w3.org/2001/XMLSchema#string"/>
  </owl:DatatypeProperty>
  <owl:DatatypeProperty rdf:about="http://example.org/onto/prop/google_clouddeploy_automation_service_account">
    <rdfs:label>service_account</rdfs:label>
    <rdfs:comment>Required. Email address of the user-managed IAM service account that creates Cloud Deploy release and rollout resources.</rdfs:comment>
    <rdfs:domain rdf:resource="http://example.org/onto/class/google_clouddeploy_automation"/>
    <rdfs:range rdf:resource="http://www.w3.org/2001/XMLSchema#string"/>
  </owl:DatatypeProperty>
  <owl:DatatypeProperty rdf:about="http://example.org/onto/prop/google_clouddeploy_automation_suspended">
    <rdfs:label>suspended</rdfs:label>
    <rdfs:comment>Optional. When Suspended, automation is deactivated from execution.</rdfs:comment>
    <rdfs:domain rdf:resource="http://example.org/onto/class/google_clouddeploy_automation"/>
    <rdfs:range rdf:resource="http://www.w3.org/2001/XMLSchema#string"/>
  </owl:DatatypeProperty>
  <owl:DatatypeProperty rdf:about="http://example.org/onto/prop/google_clouddeploy_automation_terraform_labels">
    <rdfs:label>terraform_labels</rdfs:label>
    <rdfs:comment>The combination of labels configured directly on the resource
 and default labels configured on the provider.</rdfs:comment>
    <rdfs:domain rdf:resource="http://example.org/onto/class/google_clouddeploy_automation"/>
    <rdfs:range rdf:resource="http://www.w3.org/2001/XMLSchema#string"/>
  </owl:DatatypeProperty>
  <owl:DatatypeProperty rdf:about="http://example.org/onto/prop/google_clouddeploy_automation_uid">
    <rdfs:label>uid</rdfs:label>
    <rdfs:comment>Output only. Unique identifier of the 'Automation'.</rdfs:comment>
    <rdfs:domain rdf:resource="http://example.org/onto/class/google_clouddeploy_automation"/>
    <rdfs:range rdf:resource="http://www.w3.org/2001/XMLSchema#string"/>
  </owl:DatatypeProperty>
  <owl:DatatypeProperty rdf:about="http://example.org/onto/prop/google_clouddeploy_automation_update_time">
    <rdfs:label>update_time</rdfs:label>
    <rdfs:comment>Output only. Time at which the automation was updated.</rdfs:comment>
    <rdfs:domain rdf:resource="http://example.org/onto/class/google_clouddeploy_automation"/>
    <rdfs:range rdf:resource="http://www.w3.org/2001/XMLSchema#string"/>
  </owl:DatatypeProperty>
  <owl:DatatypeProperty rdf:about="http://example.org/onto/prop/google_clouddeploy_automation_id">
    <rdfs:label>id</rdfs:label>
    <rdfs:comment>Required. ID of the rule. This id must be unique in the 'Automation' resource to which this rule belongs. The format is 'a-z{0,62}'.</rdfs:comment>
    <rdfs:domain rdf:resource="http://example.org/onto/class/google_clouddeploy_automation"/>
    <rdfs:range rdf:resource="http://www.w3.org/2001/XMLSchema#string"/>
  </owl:DatatypeProperty>
  <owl:DatatypeProperty rdf:about="http://example.org/onto/prop/google_clouddeploy_automation_source_phases">
    <rdfs:label>source_phases</rdfs:label>
    <rdfs:comment>Optional. Proceeds only after phase name matched any one in the list. This value must consist of lower-case letters, numbers, and hyphens, start with a letter and end with a letter or a number, and have a max length of 63 characters. In other words, it must match the following regex: '^[a-z]([a-z0-9-]{0,61}[a-z0-9])?$'.</rdfs:comment>
    <rdfs:domain rdf:resource="http://example.org/onto/class/google_clouddeploy_automation"/>
    <rdfs:range rdf:resource="http://www.w3.org/2001/XMLSchema#string"/>
  </owl:DatatypeProperty>
  <owl:DatatypeProperty rdf:about="http://example.org/onto/prop/google_clouddeploy_automation_wait">
    <rdfs:label>wait</rdfs:label>
    <rdfs:comment>Optional. How long to wait after a rollout is finished.</rdfs:comment>
    <rdfs:domain rdf:resource="http://example.org/onto/class/google_clouddeploy_automation"/>
    <rdfs:range rdf:resource="http://www.w3.org/2001/XMLSchema#string"/>
  </owl:DatatypeProperty>
  <owl:DatatypeProperty rdf:about="http://example.org/onto/prop/google_clouddeploy_automation_destination_phase">
    <rdfs:label>destination_phase</rdfs:label>
    <rdfs:comment>Optional. The starting phase of the rollout created by this operation. Default to the first phase.</rdfs:comment>
    <rdfs:domain rdf:resource="http://example.org/onto/class/google_clouddeploy_automation"/>
    <rdfs:range rdf:resource="http://www.w3.org/2001/XMLSchema#string"/>
  </owl:DatatypeProperty>
  <owl:DatatypeProperty rdf:about="http://example.org/onto/prop/google_clouddeploy_automation_destination_target_id">
    <rdfs:label>destination_target_id</rdfs:label>
    <rdfs:comment>Optional. The ID of the stage in the pipeline to which this 'Release' is deploying. If unspecified, default it to the next stage in the promotion flow. The value of this field could be one of the following: * The last segment of a target name. It only needs the ID to determine if the target is one of the stages in the promotion sequence defined in the pipeline. * "@next", the next target in the promotion sequence.</rdfs:comment>
    <rdfs:domain rdf:resource="http://example.org/onto/class/google_clouddeploy_automation"/>
    <rdfs:range rdf:resource="http://www.w3.org/2001/XMLSchema#string"/>
  </owl:DatatypeProperty>
  <owl:DatatypeProperty rdf:about="http://example.org/onto/prop/google_clouddeploy_automation_id">
    <rdfs:label>id</rdfs:label>
    <rdfs:comment>Required. ID of the rule. This id must be unique in the 'Automation' resource to which this rule belongs. The format is 'a-z{0,62}'.</rdfs:comment>
    <rdfs:domain rdf:resource="http://example.org/onto/class/google_clouddeploy_automation"/>
    <rdfs:range rdf:resource="http://www.w3.org/2001/XMLSchema#string"/>
  </owl:DatatypeProperty>
  <owl:DatatypeProperty rdf:about="http://example.org/onto/prop/google_clouddeploy_automation_wait">
    <rdfs:label>wait</rdfs:label>
    <rdfs:comment>Optional. How long the release need to be paused until being promoted to the next target.</rdfs:comment>
    <rdfs:domain rdf:resource="http://example.org/onto/class/google_clouddeploy_automation"/>
    <rdfs:range rdf:resource="http://www.w3.org/2001/XMLSchema#string"/>
  </owl:DatatypeProperty>
  <owl:DatatypeProperty rdf:about="http://example.org/onto/prop/google_clouddeploy_automation_id">
    <rdfs:label>id</rdfs:label>
    <rdfs:comment>Required. ID of the rule. This id must be unique in the 'Automation' resource to which this rule belongs. The format is 'a-z{0,62}'.</rdfs:comment>
    <rdfs:domain rdf:resource="http://example.org/onto/class/google_clouddeploy_automation"/>
    <rdfs:range rdf:resource="http://www.w3.org/2001/XMLSchema#string"/>
  </owl:DatatypeProperty>
  <owl:DatatypeProperty rdf:about="http://example.org/onto/prop/google_clouddeploy_automation_jobs">
    <rdfs:label>jobs</rdfs:label>
    <rdfs:comment>Optional. Jobs to repair. Proceeds only after job name matched any one in the list, or for all jobs if unspecified or empty. The phase that includes the job must match the phase ID specified in sourcePhase. This value must consist of lower-case letters, numbers, and hyphens, start with a letter and end with a letter or a number, and have a max length of 63 characters. In other words, it must match the following regex: ^[a-z]([a-z0-9-]{0,61}[a-z0-9])?$.</rdfs:comment>
    <rdfs:domain rdf:resource="http://example.org/onto/class/google_clouddeploy_automation"/>
    <rdfs:range rdf:resource="http://www.w3.org/2001/XMLSchema#string"/>
  </owl:DatatypeProperty>
  <owl:DatatypeProperty rdf:about="http://example.org/onto/prop/google_clouddeploy_automation_phases">
    <rdfs:label>phases</rdfs:label>
    <rdfs:comment>Optional. Phases within which jobs are subject to automatic repair actions on failure. Proceeds only after phase name matched any one in the list, or for all phases if unspecified. This value must consist of lower-case letters, numbers, and hyphens, start with a letter and end with a letter or a number, and have a max length of 63 characters. In other words, it must match the following regex: ^[a-z]([a-z0-9-]{0,61}[a-z0-9])?$.</rdfs:comment>
    <rdfs:domain rdf:resource="http://example.org/onto/class/google_clouddeploy_automation"/>
    <rdfs:range rdf:resource="http://www.w3.org/2001/XMLSchema#string"/>
  </owl:DatatypeProperty>
  <owl:DatatypeProperty rdf:about="http://example.org/onto/prop/google_clouddeploy_automation_attempts">
    <rdfs:label>attempts</rdfs:label>
    <rdfs:comment>Required. Total number of retries. Retry is skipped if set to 0; The minimum value is 1, and the maximum value is 10.</rdfs:comment>
    <rdfs:domain rdf:resource="http://example.org/onto/class/google_clouddeploy_automation"/>
    <rdfs:range rdf:resource="http://www.w3.org/2001/XMLSchema#string"/>
  </owl:DatatypeProperty>
  <owl:DatatypeProperty rdf:about="http://example.org/onto/prop/google_clouddeploy_automation_backoff_mode">
    <rdfs:label>backoff_mode</rdfs:label>
    <rdfs:comment>Optional. The pattern of how wait time will be increased. Default is linear. Backoff mode will be ignored if wait is 0. Possible values: ["BACKOFF_MODE_UNSPECIFIED", "BACKOFF_MODE_LINEAR", "BACKOFF_MODE_EXPONENTIAL"]</rdfs:comment>
    <rdfs:domain rdf:resource="http://example.org/onto/class/google_clouddeploy_automation"/>
    <rdfs:range rdf:resource="http://www.w3.org/2001/XMLSchema#string"/>
  </owl:DatatypeProperty>
  <owl:DatatypeProperty rdf:about="http://example.org/onto/prop/google_clouddeploy_automation_wait">
    <rdfs:label>wait</rdfs:label>
    <rdfs:comment>Optional. How long to wait for the first retry. Default is 0, and the maximum value is 14d. A duration in seconds with up to nine fractional digits, ending with 's'. Example: '3.5s'.</rdfs:comment>
    <rdfs:domain rdf:resource="http://example.org/onto/class/google_clouddeploy_automation"/>
    <rdfs:range rdf:resource="http://www.w3.org/2001/XMLSchema#string"/>
  </owl:DatatypeProperty>
  <owl:DatatypeProperty rdf:about="http://example.org/onto/prop/google_clouddeploy_automation_destination_phase">
    <rdfs:label>destination_phase</rdfs:label>
    <rdfs:comment>Optional. The starting phase ID for the Rollout. If unspecified, the Rollout will start in the stable phase.</rdfs:comment>
    <rdfs:domain rdf:resource="http://example.org/onto/class/google_clouddeploy_automation"/>
    <rdfs:range rdf:resource="http://www.w3.org/2001/XMLSchema#string"/>
  </owl:DatatypeProperty>
  <owl:DatatypeProperty rdf:about="http://example.org/onto/prop/google_clouddeploy_automation_disable_rollback_if_rollout_pending">
    <rdfs:label>disable_rollback_if_rollout_pending</rdfs:label>
    <rdfs:comment>Optional. If pending rollout exists on the target, the rollback operation will be aborted.</rdfs:comment>
    <rdfs:domain rdf:resource="http://example.org/onto/class/google_clouddeploy_automation"/>
    <rdfs:range rdf:resource="http://www.w3.org/2001/XMLSchema#string"/>
  </owl:DatatypeProperty>
  <owl:DatatypeProperty rdf:about="http://example.org/onto/prop/google_clouddeploy_automation_destination_phase">
    <rdfs:label>destination_phase</rdfs:label>
    <rdfs:comment>Optional. The starting phase of the rollout created by this rule. Default to the first phase.</rdfs:comment>
    <rdfs:domain rdf:resource="http://example.org/onto/class/google_clouddeploy_automation"/>
    <rdfs:range rdf:resource="http://www.w3.org/2001/XMLSchema#string"/>
  </owl:DatatypeProperty>
  <owl:DatatypeProperty rdf:about="http://example.org/onto/prop/google_clouddeploy_automation_destination_target_id">
    <rdfs:label>destination_target_id</rdfs:label>
    <rdfs:comment>Optional. The ID of the stage in the pipeline to which this Release is deploying. If unspecified, default it to the next stage in the promotion flow. The value of this field could be one of the following:
  - The last segment of a target name
  - "@next", the next target in the promotion sequence"</rdfs:comment>
    <rdfs:domain rdf:resource="http://example.org/onto/class/google_clouddeploy_automation"/>
    <rdfs:range rdf:resource="http://www.w3.org/2001/XMLSchema#string"/>
  </owl:DatatypeProperty>
  <owl:DatatypeProperty rdf:about="http://example.org/onto/prop/google_clouddeploy_automation_id">
    <rdfs:label>id</rdfs:label>
    <rdfs:comment>Required. ID of the rule. This id must be unique in the 'Automation' resource to which this rule belongs. The format is 'a-z{0,62}'.</rdfs:comment>
    <rdfs:domain rdf:resource="http://example.org/onto/class/google_clouddeploy_automation"/>
    <rdfs:range rdf:resource="http://www.w3.org/2001/XMLSchema#string"/>
  </owl:DatatypeProperty>
  <owl:DatatypeProperty rdf:about="http://example.org/onto/prop/google_clouddeploy_automation_schedule">
    <rdfs:label>schedule</rdfs:label>
    <rdfs:comment>Required. Schedule in crontab format. e.g. '0 9 * * 1' for every Monday at 9am.</rdfs:comment>
    <rdfs:domain rdf:resource="http://example.org/onto/class/google_clouddeploy_automation"/>
    <rdfs:range rdf:resource="http://www.w3.org/2001/XMLSchema#string"/>
  </owl:DatatypeProperty>
  <owl:DatatypeProperty rdf:about="http://example.org/onto/prop/google_clouddeploy_automation_time_zone">
    <rdfs:label>time_zone</rdfs:label>
    <rdfs:comment>Required. The time zone in IANA format IANA Time Zone Database (e.g. America/New_York).</rdfs:comment>
    <rdfs:domain rdf:resource="http://example.org/onto/class/google_clouddeploy_automation"/>
    <rdfs:range rdf:resource="http://www.w3.org/2001/XMLSchema#string"/>
  </owl:DatatypeProperty>
  <owl:DatatypeProperty rdf:about="http://example.org/onto/prop/google_clouddeploy_automation_id">
    <rdfs:label>id</rdfs:label>
    <rdfs:comment>ID of the 'Target'. The value of this field could be one of the following: * The last segment of a target name. It only needs the ID to determine which target is being referred to * "*", all targets in a location.</rdfs:comment>
    <rdfs:domain rdf:resource="http://example.org/onto/class/google_clouddeploy_automation"/>
    <rdfs:range rdf:resource="http://www.w3.org/2001/XMLSchema#string"/>
  </owl:DatatypeProperty>
  <owl:DatatypeProperty rdf:about="http://example.org/onto/prop/google_clouddeploy_automation_labels">
    <rdfs:label>labels</rdfs:label>
    <rdfs:comment>Target labels.</rdfs:comment>
    <rdfs:domain rdf:resource="http://example.org/onto/class/google_clouddeploy_automation"/>
    <rdfs:range rdf:resource="http://www.w3.org/2001/XMLSchema#string"/>
  </owl:DatatypeProperty>
  <owl:DatatypeProperty rdf:about="http://example.org/onto/prop/google_clouddeploy_automation_create">
    <rdfs:label>create</rdfs:label>
    <rdfs:domain rdf:resource="http://example.org/onto/class/google_clouddeploy_automation"/>
    <rdfs:range rdf:resource="http://www.w3.org/2001/XMLSchema#string"/>
  </owl:DatatypeProperty>
  <owl:DatatypeProperty rdf:about="http://example.org/onto/prop/google_clouddeploy_automation_delete">
    <rdfs:label>delete</rdfs:label>
    <rdfs:domain rdf:resource="http://example.org/onto/class/google_clouddeploy_automation"/>
    <rdfs:range rdf:resource="http://www.w3.org/2001/XMLSchema#string"/>
  </owl:DatatypeProperty>
  <owl:DatatypeProperty rdf:about="http://example.org/onto/prop/google_clouddeploy_automation_update">
    <rdfs:label>update</rdfs:label>
    <rdfs:domain rdf:resource="http://example.org/onto/class/google_clouddeploy_automation"/>
    <rdfs:range rdf:resource="http://www.w3.org/2001/XMLSchema#string"/>
  </owl:DatatypeProperty>
</rdf:RDF>
