<?xml version="1.0" encoding="UTF-8"?>
<rdf:RDF
  xmlns:rdf="http://www.w3.org/1999/02/22-rdf-syntax-ns#"
  xmlns:rdfs="http://www.w3.org/2000/01/rdf-schema#"
  xmlns:owl="http://www.w3.org/2002/07/owl#"
  xmlns:xsd="http://www.w3.org/2001/XMLSchema#"
  xml:base="http://example.org/onto/">
  <owl:Class rdf:about="http://example.org/onto/class/google_cloudbuild_trigger">
    <rdfs:label>google_cloudbuild_trigger</rdfs:label>
    <rdfs:comment>#
#     ***     AUTO GENERATED CODE    ***    Type: MMv1     ***
#
# ----------------------------------------------------------------------------
#
#     This code is generated by Magic Modules using the following:
#
#     Configuration: https:#github.com/GoogleCloudPlatform/magic-modules/tree/main/mmv1/products/cloudbuild/Trigger.yaml
#     Template:      https:#github.com/GoogleCloudPlatform/magic-modules/tree/main/mmv1/templates/terraform/resource.html.markdown.tmpl
#
#     DO NOT EDIT this file directly. Any changes made to this file will be
#     overwritten during the next generation cycle.
#
# ----------------------------------------------------------------------------
subcategory: "Cloud Build"
description: |-
  Configuration for an automated build in response to source repository changes.
---</rdfs:comment>
  </owl:Class>
  <owl:DatatypeProperty rdf:about="http://example.org/onto/prop/google_cloudbuild_trigger_create_time">
    <rdfs:label>create_time</rdfs:label>
    <rdfs:comment>Time when the trigger was created.</rdfs:comment>
    <rdfs:domain rdf:resource="http://example.org/onto/class/google_cloudbuild_trigger"/>
    <rdfs:range rdf:resource="http://www.w3.org/2001/XMLSchema#string"/>
  </owl:DatatypeProperty>
  <owl:DatatypeProperty rdf:about="http://example.org/onto/prop/google_cloudbuild_trigger_description">
    <rdfs:label>description</rdfs:label>
    <rdfs:comment>Human-readable description of the trigger.</rdfs:comment>
    <rdfs:domain rdf:resource="http://example.org/onto/class/google_cloudbuild_trigger"/>
    <rdfs:range rdf:resource="http://www.w3.org/2001/XMLSchema#string"/>
  </owl:DatatypeProperty>
  <owl:DatatypeProperty rdf:about="http://example.org/onto/prop/google_cloudbuild_trigger_disabled">
    <rdfs:label>disabled</rdfs:label>
    <rdfs:comment>Whether the trigger is disabled or not. If true, the trigger will never result in a build.</rdfs:comment>
    <rdfs:domain rdf:resource="http://example.org/onto/class/google_cloudbuild_trigger"/>
    <rdfs:range rdf:resource="http://www.w3.org/2001/XMLSchema#string"/>
  </owl:DatatypeProperty>
  <owl:DatatypeProperty rdf:about="http://example.org/onto/prop/google_cloudbuild_trigger_filename">
    <rdfs:label>filename</rdfs:label>
    <rdfs:comment>Path, from the source root, to a file whose contents is used for the template.
Either a filename or build template must be provided. Set this only when using trigger_template or github.
When using Pub/Sub, Webhook or Manual set the file name using git_file_source instead.</rdfs:comment>
    <rdfs:domain rdf:resource="http://example.org/onto/class/google_cloudbuild_trigger"/>
    <rdfs:range rdf:resource="http://www.w3.org/2001/XMLSchema#string"/>
  </owl:DatatypeProperty>
  <owl:DatatypeProperty rdf:about="http://example.org/onto/prop/google_cloudbuild_trigger_filter">
    <rdfs:label>filter</rdfs:label>
    <rdfs:comment>A Common Expression Language string. Used only with Pub/Sub and Webhook.</rdfs:comment>
    <rdfs:domain rdf:resource="http://example.org/onto/class/google_cloudbuild_trigger"/>
    <rdfs:range rdf:resource="http://www.w3.org/2001/XMLSchema#string"/>
  </owl:DatatypeProperty>
  <owl:DatatypeProperty rdf:about="http://example.org/onto/prop/google_cloudbuild_trigger_id">
    <rdfs:label>id</rdfs:label>
    <rdfs:domain rdf:resource="http://example.org/onto/class/google_cloudbuild_trigger"/>
    <rdfs:range rdf:resource="http://www.w3.org/2001/XMLSchema#string"/>
  </owl:DatatypeProperty>
  <owl:DatatypeProperty rdf:about="http://example.org/onto/prop/google_cloudbuild_trigger_ignored_files">
    <rdfs:label>ignored_files</rdfs:label>
    <rdfs:comment>ignoredFiles and includedFiles are file glob matches using https://golang.org/pkg/path/filepath/#Match
extended with support for '**'.

If ignoredFiles and changed files are both empty, then they are not
used to determine whether or not to trigger a build.

If ignoredFiles is not empty, then we ignore any files that match any
of the ignored_file globs. If the change has no files that are outside
of the ignoredFiles globs, then we do not trigger a build.</rdfs:comment>
    <rdfs:domain rdf:resource="http://example.org/onto/class/google_cloudbuild_trigger"/>
    <rdfs:range rdf:resource="http://www.w3.org/2001/XMLSchema#string"/>
  </owl:DatatypeProperty>
  <owl:DatatypeProperty rdf:about="http://example.org/onto/prop/google_cloudbuild_trigger_include_build_logs">
    <rdfs:label>include_build_logs</rdfs:label>
    <rdfs:comment>Build logs will be sent back to GitHub as part of the checkrun
result.  Values can be INCLUDE_BUILD_LOGS_UNSPECIFIED or
INCLUDE_BUILD_LOGS_WITH_STATUS Possible values: ["INCLUDE_BUILD_LOGS_UNSPECIFIED", "INCLUDE_BUILD_LOGS_WITH_STATUS"]</rdfs:comment>
    <rdfs:domain rdf:resource="http://example.org/onto/class/google_cloudbuild_trigger"/>
    <rdfs:range rdf:resource="http://www.w3.org/2001/XMLSchema#string"/>
  </owl:DatatypeProperty>
  <owl:DatatypeProperty rdf:about="http://example.org/onto/prop/google_cloudbuild_trigger_included_files">
    <rdfs:label>included_files</rdfs:label>
    <rdfs:comment>ignoredFiles and includedFiles are file glob matches using https://golang.org/pkg/path/filepath/#Match
extended with support for '**'.

If any of the files altered in the commit pass the ignoredFiles filter
and includedFiles is empty, then as far as this filter is concerned, we
should trigger the build.

If any of the files altered in the commit pass the ignoredFiles filter
and includedFiles is not empty, then we make sure that at least one of
those files matches a includedFiles glob. If not, then we do not trigger
a build.</rdfs:comment>
    <rdfs:domain rdf:resource="http://example.org/onto/class/google_cloudbuild_trigger"/>
    <rdfs:range rdf:resource="http://www.w3.org/2001/XMLSchema#string"/>
  </owl:DatatypeProperty>
  <owl:DatatypeProperty rdf:about="http://example.org/onto/prop/google_cloudbuild_trigger_location">
    <rdfs:label>location</rdfs:label>
    <rdfs:comment>The [Cloud Build location](https://cloud.google.com/build/docs/locations) for the trigger.
If not specified, "global" is used.</rdfs:comment>
    <rdfs:domain rdf:resource="http://example.org/onto/class/google_cloudbuild_trigger"/>
    <rdfs:range rdf:resource="http://www.w3.org/2001/XMLSchema#string"/>
  </owl:DatatypeProperty>
  <owl:DatatypeProperty rdf:about="http://example.org/onto/prop/google_cloudbuild_trigger_name">
    <rdfs:label>name</rdfs:label>
    <rdfs:comment>Name of the trigger. Must be unique within the project.</rdfs:comment>
    <rdfs:domain rdf:resource="http://example.org/onto/class/google_cloudbuild_trigger"/>
    <rdfs:range rdf:resource="http://www.w3.org/2001/XMLSchema#string"/>
  </owl:DatatypeProperty>
  <owl:DatatypeProperty rdf:about="http://example.org/onto/prop/google_cloudbuild_trigger_project">
    <rdfs:label>project</rdfs:label>
    <rdfs:domain rdf:resource="http://example.org/onto/class/google_cloudbuild_trigger"/>
    <rdfs:range rdf:resource="http://www.w3.org/2001/XMLSchema#string"/>
  </owl:DatatypeProperty>
  <owl:DatatypeProperty rdf:about="http://example.org/onto/prop/google_cloudbuild_trigger_service_account">
    <rdfs:label>service_account</rdfs:label>
    <rdfs:comment>The service account used for all user-controlled operations including
triggers.patch, triggers.run, builds.create, and builds.cancel.

If no service account is set, then the standard Cloud Build service account
([PROJECT_NUM]@system.gserviceaccount.com) will be used instead.

Format: projects/{PROJECT_ID}/serviceAccounts/{ACCOUNT_ID_OR_EMAIL}</rdfs:comment>
    <rdfs:domain rdf:resource="http://example.org/onto/class/google_cloudbuild_trigger"/>
    <rdfs:range rdf:resource="http://www.w3.org/2001/XMLSchema#string"/>
  </owl:DatatypeProperty>
  <owl:DatatypeProperty rdf:about="http://example.org/onto/prop/google_cloudbuild_trigger_substitutions">
    <rdfs:label>substitutions</rdfs:label>
    <rdfs:comment>Substitutions data for Build resource.</rdfs:comment>
    <rdfs:domain rdf:resource="http://example.org/onto/class/google_cloudbuild_trigger"/>
    <rdfs:range rdf:resource="http://www.w3.org/2001/XMLSchema#string"/>
  </owl:DatatypeProperty>
  <owl:DatatypeProperty rdf:about="http://example.org/onto/prop/google_cloudbuild_trigger_tags">
    <rdfs:label>tags</rdfs:label>
    <rdfs:comment>Tags for annotation of a BuildTrigger</rdfs:comment>
    <rdfs:domain rdf:resource="http://example.org/onto/class/google_cloudbuild_trigger"/>
    <rdfs:range rdf:resource="http://www.w3.org/2001/XMLSchema#string"/>
  </owl:DatatypeProperty>
  <owl:DatatypeProperty rdf:about="http://example.org/onto/prop/google_cloudbuild_trigger_trigger_id">
    <rdfs:label>trigger_id</rdfs:label>
    <rdfs:comment>The unique identifier for the trigger.</rdfs:comment>
    <rdfs:domain rdf:resource="http://example.org/onto/class/google_cloudbuild_trigger"/>
    <rdfs:range rdf:resource="http://www.w3.org/2001/XMLSchema#string"/>
  </owl:DatatypeProperty>
  <owl:DatatypeProperty rdf:about="http://example.org/onto/prop/google_cloudbuild_trigger_approval_required">
    <rdfs:label>approval_required</rdfs:label>
    <rdfs:comment>Whether or not approval is needed. If this is set on a build, it will become pending when run,
and will need to be explicitly approved to start.</rdfs:comment>
    <rdfs:domain rdf:resource="http://example.org/onto/class/google_cloudbuild_trigger"/>
    <rdfs:range rdf:resource="http://www.w3.org/2001/XMLSchema#string"/>
  </owl:DatatypeProperty>
  <owl:DatatypeProperty rdf:about="http://example.org/onto/prop/google_cloudbuild_trigger_bitbucket_server_config_resource">
    <rdfs:label>bitbucket_server_config_resource</rdfs:label>
    <rdfs:comment>The Bitbucket server config resource that this trigger config maps to.</rdfs:comment>
    <rdfs:domain rdf:resource="http://example.org/onto/class/google_cloudbuild_trigger"/>
    <rdfs:range rdf:resource="http://www.w3.org/2001/XMLSchema#string"/>
  </owl:DatatypeProperty>
  <owl:DatatypeProperty rdf:about="http://example.org/onto/prop/google_cloudbuild_trigger_project_key">
    <rdfs:label>project_key</rdfs:label>
    <rdfs:comment>Key of the project that the repo is in. For example: The key for https://mybitbucket.server/projects/TEST/repos/test-repo is "TEST".</rdfs:comment>
    <rdfs:domain rdf:resource="http://example.org/onto/class/google_cloudbuild_trigger"/>
    <rdfs:range rdf:resource="http://www.w3.org/2001/XMLSchema#string"/>
  </owl:DatatypeProperty>
  <owl:DatatypeProperty rdf:about="http://example.org/onto/prop/google_cloudbuild_trigger_repo_slug">
    <rdfs:label>repo_slug</rdfs:label>
    <rdfs:comment>Slug of the repository. A repository slug is a URL-friendly version of a repository name, automatically generated by Bitbucket for use in the URL.
For example, if the repository name is 'test repo', in the URL it would become 'test-repo' as in https://mybitbucket.server/projects/TEST/repos/test-repo.</rdfs:comment>
    <rdfs:domain rdf:resource="http://example.org/onto/class/google_cloudbuild_trigger"/>
    <rdfs:range rdf:resource="http://www.w3.org/2001/XMLSchema#string"/>
  </owl:DatatypeProperty>
  <owl:DatatypeProperty rdf:about="http://example.org/onto/prop/google_cloudbuild_trigger_branch">
    <rdfs:label>branch</rdfs:label>
    <rdfs:comment>Regex of branches to match.
The syntax of the regular expressions accepted is the syntax accepted by RE2 and described at https://github.com/google/re2/wiki/Syntax</rdfs:comment>
    <rdfs:domain rdf:resource="http://example.org/onto/class/google_cloudbuild_trigger"/>
    <rdfs:range rdf:resource="http://www.w3.org/2001/XMLSchema#string"/>
  </owl:DatatypeProperty>
  <owl:DatatypeProperty rdf:about="http://example.org/onto/prop/google_cloudbuild_trigger_comment_control">
    <rdfs:label>comment_control</rdfs:label>
    <rdfs:comment>Configure builds to run whether a repository owner or collaborator need to comment /gcbrun. Possible values: ["COMMENTS_DISABLED", "COMMENTS_ENABLED", "COMMENTS_ENABLED_FOR_EXTERNAL_CONTRIBUTORS_ONLY"]</rdfs:comment>
    <rdfs:domain rdf:resource="http://example.org/onto/class/google_cloudbuild_trigger"/>
    <rdfs:range rdf:resource="http://www.w3.org/2001/XMLSchema#string"/>
  </owl:DatatypeProperty>
  <owl:DatatypeProperty rdf:about="http://example.org/onto/prop/google_cloudbuild_trigger_invert_regex">
    <rdfs:label>invert_regex</rdfs:label>
    <rdfs:comment>If true, branches that do NOT match the git_ref will trigger a build.</rdfs:comment>
    <rdfs:domain rdf:resource="http://example.org/onto/class/google_cloudbuild_trigger"/>
    <rdfs:range rdf:resource="http://www.w3.org/2001/XMLSchema#string"/>
  </owl:DatatypeProperty>
  <owl:DatatypeProperty rdf:about="http://example.org/onto/prop/google_cloudbuild_trigger_branch">
    <rdfs:label>branch</rdfs:label>
    <rdfs:comment>Regex of branches to match.  Specify only one of branch or tag.</rdfs:comment>
    <rdfs:domain rdf:resource="http://example.org/onto/class/google_cloudbuild_trigger"/>
    <rdfs:range rdf:resource="http://www.w3.org/2001/XMLSchema#string"/>
  </owl:DatatypeProperty>
  <owl:DatatypeProperty rdf:about="http://example.org/onto/prop/google_cloudbuild_trigger_invert_regex">
    <rdfs:label>invert_regex</rdfs:label>
    <rdfs:comment>When true, only trigger a build if the revision regex does NOT match the gitRef regex.</rdfs:comment>
    <rdfs:domain rdf:resource="http://example.org/onto/class/google_cloudbuild_trigger"/>
    <rdfs:range rdf:resource="http://www.w3.org/2001/XMLSchema#string"/>
  </owl:DatatypeProperty>
  <owl:DatatypeProperty rdf:about="http://example.org/onto/prop/google_cloudbuild_trigger_tag">
    <rdfs:label>tag</rdfs:label>
    <rdfs:comment>Regex of tags to match.  Specify only one of branch or tag.</rdfs:comment>
    <rdfs:domain rdf:resource="http://example.org/onto/class/google_cloudbuild_trigger"/>
    <rdfs:range rdf:resource="http://www.w3.org/2001/XMLSchema#string"/>
  </owl:DatatypeProperty>
  <owl:DatatypeProperty rdf:about="http://example.org/onto/prop/google_cloudbuild_trigger_images">
    <rdfs:label>images</rdfs:label>
    <rdfs:comment>A list of images to be pushed upon the successful completion of all build steps.
The images are pushed using the builder service account's credentials.
The digests of the pushed images will be stored in the Build resource's results field.
If any of the images fail to be pushed, the build status is marked FAILURE.</rdfs:comment>
    <rdfs:domain rdf:resource="http://example.org/onto/class/google_cloudbuild_trigger"/>
    <rdfs:range rdf:resource="http://www.w3.org/2001/XMLSchema#string"/>
  </owl:DatatypeProperty>
  <owl:DatatypeProperty rdf:about="http://example.org/onto/prop/google_cloudbuild_trigger_logs_bucket">
    <rdfs:label>logs_bucket</rdfs:label>
    <rdfs:comment>Google Cloud Storage bucket where logs should be written.
Logs file names will be of the format ${logsBucket}/log-${build_id}.txt.</rdfs:comment>
    <rdfs:domain rdf:resource="http://example.org/onto/class/google_cloudbuild_trigger"/>
    <rdfs:range rdf:resource="http://www.w3.org/2001/XMLSchema#string"/>
  </owl:DatatypeProperty>
  <owl:DatatypeProperty rdf:about="http://example.org/onto/prop/google_cloudbuild_trigger_queue_ttl">
    <rdfs:label>queue_ttl</rdfs:label>
    <rdfs:comment>TTL in queue for this build. If provided and the build is enqueued longer than this value,
the build will expire and the build status will be EXPIRED.
The TTL starts ticking from createTime.
A duration in seconds with up to nine fractional digits, terminated by 's'. Example: "3.5s".</rdfs:comment>
    <rdfs:domain rdf:resource="http://example.org/onto/class/google_cloudbuild_trigger"/>
    <rdfs:range rdf:resource="http://www.w3.org/2001/XMLSchema#string"/>
  </owl:DatatypeProperty>
  <owl:DatatypeProperty rdf:about="http://example.org/onto/prop/google_cloudbuild_trigger_substitutions">
    <rdfs:label>substitutions</rdfs:label>
    <rdfs:comment>Substitutions data for Build resource.</rdfs:comment>
    <rdfs:domain rdf:resource="http://example.org/onto/class/google_cloudbuild_trigger"/>
    <rdfs:range rdf:resource="http://www.w3.org/2001/XMLSchema#string"/>
  </owl:DatatypeProperty>
  <owl:DatatypeProperty rdf:about="http://example.org/onto/prop/google_cloudbuild_trigger_tags">
    <rdfs:label>tags</rdfs:label>
    <rdfs:comment>Tags for annotation of a Build. These are not docker tags.</rdfs:comment>
    <rdfs:domain rdf:resource="http://example.org/onto/class/google_cloudbuild_trigger"/>
    <rdfs:range rdf:resource="http://www.w3.org/2001/XMLSchema#string"/>
  </owl:DatatypeProperty>
  <owl:DatatypeProperty rdf:about="http://example.org/onto/prop/google_cloudbuild_trigger_timeout">
    <rdfs:label>timeout</rdfs:label>
    <rdfs:comment>Amount of time that this build should be allowed to run, to second granularity.
If this amount of time elapses, work on the build will cease and the build status will be TIMEOUT.
This timeout must be equal to or greater than the sum of the timeouts for build steps within the build.
The expected format is the number of seconds followed by s.
Default time is ten minutes (600s).</rdfs:comment>
    <rdfs:domain rdf:resource="http://example.org/onto/class/google_cloudbuild_trigger"/>
    <rdfs:range rdf:resource="http://www.w3.org/2001/XMLSchema#string"/>
  </owl:DatatypeProperty>
  <owl:DatatypeProperty rdf:about="http://example.org/onto/prop/google_cloudbuild_trigger_images">
    <rdfs:label>images</rdfs:label>
    <rdfs:comment>A list of images to be pushed upon the successful completion of all build steps.

The images will be pushed using the builder service account's credentials.

The digests of the pushed images will be stored in the Build resource's results field.

If any of the images fail to be pushed, the build is marked FAILURE.</rdfs:comment>
    <rdfs:domain rdf:resource="http://example.org/onto/class/google_cloudbuild_trigger"/>
    <rdfs:range rdf:resource="http://www.w3.org/2001/XMLSchema#string"/>
  </owl:DatatypeProperty>
  <owl:DatatypeProperty rdf:about="http://example.org/onto/prop/google_cloudbuild_trigger_artifact_id">
    <rdfs:label>artifact_id</rdfs:label>
    <rdfs:comment>Maven artifactId value used when uploading the artifact to Artifact Registry.</rdfs:comment>
    <rdfs:domain rdf:resource="http://example.org/onto/class/google_cloudbuild_trigger"/>
    <rdfs:range rdf:resource="http://www.w3.org/2001/XMLSchema#string"/>
  </owl:DatatypeProperty>
  <owl:DatatypeProperty rdf:about="http://example.org/onto/prop/google_cloudbuild_trigger_group_id">
    <rdfs:label>group_id</rdfs:label>
    <rdfs:comment>Maven groupId value used when uploading the artifact to Artifact Registry.</rdfs:comment>
    <rdfs:domain rdf:resource="http://example.org/onto/class/google_cloudbuild_trigger"/>
    <rdfs:range rdf:resource="http://www.w3.org/2001/XMLSchema#string"/>
  </owl:DatatypeProperty>
  <owl:DatatypeProperty rdf:about="http://example.org/onto/prop/google_cloudbuild_trigger_path">
    <rdfs:label>path</rdfs:label>
    <rdfs:comment>Path to an artifact in the build's workspace to be uploaded to Artifact Registry. This can be either an absolute path, e.g. /workspace/my-app/target/my-app-1.0.SNAPSHOT.jar or a relative path from /workspace, e.g. my-app/target/my-app-1.0.SNAPSHOT.jar.</rdfs:comment>
    <rdfs:domain rdf:resource="http://example.org/onto/class/google_cloudbuild_trigger"/>
    <rdfs:range rdf:resource="http://www.w3.org/2001/XMLSchema#string"/>
  </owl:DatatypeProperty>
  <owl:DatatypeProperty rdf:about="http://example.org/onto/prop/google_cloudbuild_trigger_repository">
    <rdfs:label>repository</rdfs:label>
    <rdfs:comment>Artifact Registry repository, in the form "https://$REGION-maven.pkg.dev/$PROJECT/$REPOSITORY"

Artifact in the workspace specified by path will be uploaded to Artifact Registry with this location as a prefix.</rdfs:comment>
    <rdfs:domain rdf:resource="http://example.org/onto/class/google_cloudbuild_trigger"/>
    <rdfs:range rdf:resource="http://www.w3.org/2001/XMLSchema#string"/>
  </owl:DatatypeProperty>
  <owl:DatatypeProperty rdf:about="http://example.org/onto/prop/google_cloudbuild_trigger_version">
    <rdfs:label>version</rdfs:label>
    <rdfs:comment>Maven version value used when uploading the artifact to Artifact Registry.</rdfs:comment>
    <rdfs:domain rdf:resource="http://example.org/onto/class/google_cloudbuild_trigger"/>
    <rdfs:range rdf:resource="http://www.w3.org/2001/XMLSchema#string"/>
  </owl:DatatypeProperty>
  <owl:DatatypeProperty rdf:about="http://example.org/onto/prop/google_cloudbuild_trigger_package_path">
    <rdfs:label>package_path</rdfs:label>
    <rdfs:comment>Path to the package.json. e.g. workspace/path/to/package</rdfs:comment>
    <rdfs:domain rdf:resource="http://example.org/onto/class/google_cloudbuild_trigger"/>
    <rdfs:range rdf:resource="http://www.w3.org/2001/XMLSchema#string"/>
  </owl:DatatypeProperty>
  <owl:DatatypeProperty rdf:about="http://example.org/onto/prop/google_cloudbuild_trigger_repository">
    <rdfs:label>repository</rdfs:label>
    <rdfs:comment>Artifact Registry repository, in the form "https://$REGION-npm.pkg.dev/$PROJECT/$REPOSITORY"

Npm package in the workspace specified by path will be zipped and uploaded to Artifact Registry with this location as a prefix.</rdfs:comment>
    <rdfs:domain rdf:resource="http://example.org/onto/class/google_cloudbuild_trigger"/>
    <rdfs:range rdf:resource="http://www.w3.org/2001/XMLSchema#string"/>
  </owl:DatatypeProperty>
  <owl:DatatypeProperty rdf:about="http://example.org/onto/prop/google_cloudbuild_trigger_location">
    <rdfs:label>location</rdfs:label>
    <rdfs:comment>Cloud Storage bucket and optional object path, in the form "gs://bucket/path/to/somewhere/".

Files in the workspace matching any path pattern will be uploaded to Cloud Storage with
this location as a prefix.</rdfs:comment>
    <rdfs:domain rdf:resource="http://example.org/onto/class/google_cloudbuild_trigger"/>
    <rdfs:range rdf:resource="http://www.w3.org/2001/XMLSchema#string"/>
  </owl:DatatypeProperty>
  <owl:DatatypeProperty rdf:about="http://example.org/onto/prop/google_cloudbuild_trigger_paths">
    <rdfs:label>paths</rdfs:label>
    <rdfs:comment>Path globs used to match files in the build's workspace.</rdfs:comment>
    <rdfs:domain rdf:resource="http://example.org/onto/class/google_cloudbuild_trigger"/>
    <rdfs:range rdf:resource="http://www.w3.org/2001/XMLSchema#string"/>
  </owl:DatatypeProperty>
  <owl:DatatypeProperty rdf:about="http://example.org/onto/prop/google_cloudbuild_trigger_timing">
    <rdfs:label>timing</rdfs:label>
    <rdfs:comment>Output only. Stores timing information for pushing all artifact objects.</rdfs:comment>
    <rdfs:domain rdf:resource="http://example.org/onto/class/google_cloudbuild_trigger"/>
    <rdfs:range rdf:resource="http://www.w3.org/2001/XMLSchema#string"/>
  </owl:DatatypeProperty>
  <owl:DatatypeProperty rdf:about="http://example.org/onto/prop/google_cloudbuild_trigger_paths">
    <rdfs:label>paths</rdfs:label>
    <rdfs:comment>Path globs used to match files in the build's workspace. For Python/ Twine, this is usually dist/*, and sometimes additionally an .asc file.</rdfs:comment>
    <rdfs:domain rdf:resource="http://example.org/onto/class/google_cloudbuild_trigger"/>
    <rdfs:range rdf:resource="http://www.w3.org/2001/XMLSchema#string"/>
  </owl:DatatypeProperty>
  <owl:DatatypeProperty rdf:about="http://example.org/onto/prop/google_cloudbuild_trigger_repository">
    <rdfs:label>repository</rdfs:label>
    <rdfs:comment>Artifact Registry repository, in the form "https://$REGION-python.pkg.dev/$PROJECT/$REPOSITORY"

Files in the workspace matching any path pattern will be uploaded to Artifact Registry with this location as a prefix.</rdfs:comment>
    <rdfs:domain rdf:resource="http://example.org/onto/class/google_cloudbuild_trigger"/>
    <rdfs:range rdf:resource="http://www.w3.org/2001/XMLSchema#string"/>
  </owl:DatatypeProperty>
  <owl:DatatypeProperty rdf:about="http://example.org/onto/prop/google_cloudbuild_trigger_env">
    <rdfs:label>env</rdfs:label>
    <rdfs:comment>Environment variable name to associate with the secret. Secret environment
variables must be unique across all of a build's secrets, and must be used
by at least one build step.</rdfs:comment>
    <rdfs:domain rdf:resource="http://example.org/onto/class/google_cloudbuild_trigger"/>
    <rdfs:range rdf:resource="http://www.w3.org/2001/XMLSchema#string"/>
  </owl:DatatypeProperty>
  <owl:DatatypeProperty rdf:about="http://example.org/onto/prop/google_cloudbuild_trigger_version_name">
    <rdfs:label>version_name</rdfs:label>
    <rdfs:comment>Resource name of the SecretVersion. In format: projects/*/secrets/*/versions/*</rdfs:comment>
    <rdfs:domain rdf:resource="http://example.org/onto/class/google_cloudbuild_trigger"/>
    <rdfs:range rdf:resource="http://www.w3.org/2001/XMLSchema#string"/>
  </owl:DatatypeProperty>
  <owl:DatatypeProperty rdf:about="http://example.org/onto/prop/google_cloudbuild_trigger_disk_size_gb">
    <rdfs:label>disk_size_gb</rdfs:label>
    <rdfs:comment>Requested disk size for the VM that runs the build. Note that this is NOT "disk free";
some of the space will be used by the operating system and build utilities.
Also note that this is the minimum disk size that will be allocated for the build --
the build may run with a larger disk than requested. At present, the maximum disk size
is 1000GB; builds that request more than the maximum are rejected with an error.</rdfs:comment>
    <rdfs:domain rdf:resource="http://example.org/onto/class/google_cloudbuild_trigger"/>
    <rdfs:range rdf:resource="http://www.w3.org/2001/XMLSchema#string"/>
  </owl:DatatypeProperty>
  <owl:DatatypeProperty rdf:about="http://example.org/onto/prop/google_cloudbuild_trigger_dynamic_substitutions">
    <rdfs:label>dynamic_substitutions</rdfs:label>
    <rdfs:comment>Option to specify whether or not to apply bash style string operations to the substitutions.

NOTE this is always enabled for triggered builds and cannot be overridden in the build configuration file.</rdfs:comment>
    <rdfs:domain rdf:resource="http://example.org/onto/class/google_cloudbuild_trigger"/>
    <rdfs:range rdf:resource="http://www.w3.org/2001/XMLSchema#string"/>
  </owl:DatatypeProperty>
  <owl:DatatypeProperty rdf:about="http://example.org/onto/prop/google_cloudbuild_trigger_env">
    <rdfs:label>env</rdfs:label>
    <rdfs:comment>A list of global environment variable definitions that will exist for all build steps
in this build. If a variable is defined in both globally and in a build step,
the variable will use the build step value.

The elements are of the form "KEY=VALUE" for the environment variable "KEY" being given the value "VALUE".</rdfs:comment>
    <rdfs:domain rdf:resource="http://example.org/onto/class/google_cloudbuild_trigger"/>
    <rdfs:range rdf:resource="http://www.w3.org/2001/XMLSchema#string"/>
  </owl:DatatypeProperty>
  <owl:DatatypeProperty rdf:about="http://example.org/onto/prop/google_cloudbuild_trigger_log_streaming_option">
    <rdfs:label>log_streaming_option</rdfs:label>
    <rdfs:comment>Option to define build log streaming behavior to Google Cloud Storage. Possible values: ["STREAM_DEFAULT", "STREAM_ON", "STREAM_OFF"]</rdfs:comment>
    <rdfs:domain rdf:resource="http://example.org/onto/class/google_cloudbuild_trigger"/>
    <rdfs:range rdf:resource="http://www.w3.org/2001/XMLSchema#string"/>
  </owl:DatatypeProperty>
  <owl:DatatypeProperty rdf:about="http://example.org/onto/prop/google_cloudbuild_trigger_logging">
    <rdfs:label>logging</rdfs:label>
    <rdfs:comment>Option to specify the logging mode, which determines if and where build logs are stored. Possible values: ["LOGGING_UNSPECIFIED", "LEGACY", "GCS_ONLY", "STACKDRIVER_ONLY", "CLOUD_LOGGING_ONLY", "NONE"]</rdfs:comment>
    <rdfs:domain rdf:resource="http://example.org/onto/class/google_cloudbuild_trigger"/>
    <rdfs:range rdf:resource="http://www.w3.org/2001/XMLSchema#string"/>
  </owl:DatatypeProperty>
  <owl:DatatypeProperty rdf:about="http://example.org/onto/prop/google_cloudbuild_trigger_machine_type">
    <rdfs:label>machine_type</rdfs:label>
    <rdfs:comment>Compute Engine machine type on which to run the build.</rdfs:comment>
    <rdfs:domain rdf:resource="http://example.org/onto/class/google_cloudbuild_trigger"/>
    <rdfs:range rdf:resource="http://www.w3.org/2001/XMLSchema#string"/>
  </owl:DatatypeProperty>
  <owl:DatatypeProperty rdf:about="http://example.org/onto/prop/google_cloudbuild_trigger_requested_verify_option">
    <rdfs:label>requested_verify_option</rdfs:label>
    <rdfs:comment>Requested verifiability options. Possible values: ["NOT_VERIFIED", "VERIFIED"]</rdfs:comment>
    <rdfs:domain rdf:resource="http://example.org/onto/class/google_cloudbuild_trigger"/>
    <rdfs:range rdf:resource="http://www.w3.org/2001/XMLSchema#string"/>
  </owl:DatatypeProperty>
  <owl:DatatypeProperty rdf:about="http://example.org/onto/prop/google_cloudbuild_trigger_secret_env">
    <rdfs:label>secret_env</rdfs:label>
    <rdfs:comment>A list of global environment variables, which are encrypted using a Cloud Key Management
Service crypto key. These values must be specified in the build's Secret. These variables
will be available to all build steps in this build.</rdfs:comment>
    <rdfs:domain rdf:resource="http://example.org/onto/class/google_cloudbuild_trigger"/>
    <rdfs:range rdf:resource="http://www.w3.org/2001/XMLSchema#string"/>
  </owl:DatatypeProperty>
  <owl:DatatypeProperty rdf:about="http://example.org/onto/prop/google_cloudbuild_trigger_source_provenance_hash">
    <rdfs:label>source_provenance_hash</rdfs:label>
    <rdfs:comment>Requested hash for SourceProvenance. Possible values: ["NONE", "SHA256", "MD5"]</rdfs:comment>
    <rdfs:domain rdf:resource="http://example.org/onto/class/google_cloudbuild_trigger"/>
    <rdfs:range rdf:resource="http://www.w3.org/2001/XMLSchema#string"/>
  </owl:DatatypeProperty>
  <owl:DatatypeProperty rdf:about="http://example.org/onto/prop/google_cloudbuild_trigger_substitution_option">
    <rdfs:label>substitution_option</rdfs:label>
    <rdfs:comment>Option to specify behavior when there is an error in the substitution checks.

NOTE this is always set to ALLOW_LOOSE for triggered builds and cannot be overridden
in the build configuration file. Possible values: ["MUST_MATCH", "ALLOW_LOOSE"]</rdfs:comment>
    <rdfs:domain rdf:resource="http://example.org/onto/class/google_cloudbuild_trigger"/>
    <rdfs:range rdf:resource="http://www.w3.org/2001/XMLSchema#string"/>
  </owl:DatatypeProperty>
  <owl:DatatypeProperty rdf:about="http://example.org/onto/prop/google_cloudbuild_trigger_worker_pool">
    <rdfs:label>worker_pool</rdfs:label>
    <rdfs:comment>Option to specify a WorkerPool for the build. Format projects/{project}/workerPools/{workerPool}

This field is experimental.</rdfs:comment>
    <rdfs:domain rdf:resource="http://example.org/onto/class/google_cloudbuild_trigger"/>
    <rdfs:range rdf:resource="http://www.w3.org/2001/XMLSchema#string"/>
  </owl:DatatypeProperty>
  <owl:DatatypeProperty rdf:about="http://example.org/onto/prop/google_cloudbuild_trigger_name">
    <rdfs:label>name</rdfs:label>
    <rdfs:comment>Name of the volume to mount.

Volume names must be unique per build step and must be valid names for Docker volumes.
Each named volume must be used by at least two build steps.</rdfs:comment>
    <rdfs:domain rdf:resource="http://example.org/onto/class/google_cloudbuild_trigger"/>
    <rdfs:range rdf:resource="http://www.w3.org/2001/XMLSchema#string"/>
  </owl:DatatypeProperty>
  <owl:DatatypeProperty rdf:about="http://example.org/onto/prop/google_cloudbuild_trigger_path">
    <rdfs:label>path</rdfs:label>
    <rdfs:comment>Path at which to mount the volume.

Paths must be absolute and cannot conflict with other volume paths on the same
build step or with certain reserved volume paths.</rdfs:comment>
    <rdfs:domain rdf:resource="http://example.org/onto/class/google_cloudbuild_trigger"/>
    <rdfs:range rdf:resource="http://www.w3.org/2001/XMLSchema#string"/>
  </owl:DatatypeProperty>
  <owl:DatatypeProperty rdf:about="http://example.org/onto/prop/google_cloudbuild_trigger_kms_key_name">
    <rdfs:label>kms_key_name</rdfs:label>
    <rdfs:comment>Cloud KMS key name to use to decrypt these envs.</rdfs:comment>
    <rdfs:domain rdf:resource="http://example.org/onto/class/google_cloudbuild_trigger"/>
    <rdfs:range rdf:resource="http://www.w3.org/2001/XMLSchema#string"/>
  </owl:DatatypeProperty>
  <owl:DatatypeProperty rdf:about="http://example.org/onto/prop/google_cloudbuild_trigger_secret_env">
    <rdfs:label>secret_env</rdfs:label>
    <rdfs:comment>Map of environment variable name to its encrypted value.
Secret environment variables must be unique across all of a build's secrets,
and must be used by at least one build step. Values can be at most 64 KB in size.
There can be at most 100 secret values across all of a build's secrets.</rdfs:comment>
    <rdfs:domain rdf:resource="http://example.org/onto/class/google_cloudbuild_trigger"/>
    <rdfs:range rdf:resource="http://www.w3.org/2001/XMLSchema#string"/>
  </owl:DatatypeProperty>
  <owl:DatatypeProperty rdf:about="http://example.org/onto/prop/google_cloudbuild_trigger_branch_name">
    <rdfs:label>branch_name</rdfs:label>
    <rdfs:comment>Regex matching branches to build. Exactly one a of branch name, tag, or commit SHA must be provided.
The syntax of the regular expressions accepted is the syntax accepted by RE2 and
described at https://github.com/google/re2/wiki/Syntax</rdfs:comment>
    <rdfs:domain rdf:resource="http://example.org/onto/class/google_cloudbuild_trigger"/>
    <rdfs:range rdf:resource="http://www.w3.org/2001/XMLSchema#string"/>
  </owl:DatatypeProperty>
  <owl:DatatypeProperty rdf:about="http://example.org/onto/prop/google_cloudbuild_trigger_commit_sha">
    <rdfs:label>commit_sha</rdfs:label>
    <rdfs:comment>Explicit commit SHA to build. Exactly one a of branch name, tag, or commit SHA must be provided.</rdfs:comment>
    <rdfs:domain rdf:resource="http://example.org/onto/class/google_cloudbuild_trigger"/>
    <rdfs:range rdf:resource="http://www.w3.org/2001/XMLSchema#string"/>
  </owl:DatatypeProperty>
  <owl:DatatypeProperty rdf:about="http://example.org/onto/prop/google_cloudbuild_trigger_dir">
    <rdfs:label>dir</rdfs:label>
    <rdfs:comment>Directory, relative to the source root, in which to run the build.
This must be a relative path. If a step's dir is specified and is an absolute path,
this value is ignored for that step's execution.</rdfs:comment>
    <rdfs:domain rdf:resource="http://example.org/onto/class/google_cloudbuild_trigger"/>
    <rdfs:range rdf:resource="http://www.w3.org/2001/XMLSchema#string"/>
  </owl:DatatypeProperty>
  <owl:DatatypeProperty rdf:about="http://example.org/onto/prop/google_cloudbuild_trigger_invert_regex">
    <rdfs:label>invert_regex</rdfs:label>
    <rdfs:comment>Only trigger a build if the revision regex does NOT match the revision regex.</rdfs:comment>
    <rdfs:domain rdf:resource="http://example.org/onto/class/google_cloudbuild_trigger"/>
    <rdfs:range rdf:resource="http://www.w3.org/2001/XMLSchema#string"/>
  </owl:DatatypeProperty>
  <owl:DatatypeProperty rdf:about="http://example.org/onto/prop/google_cloudbuild_trigger_project_id">
    <rdfs:label>project_id</rdfs:label>
    <rdfs:comment>ID of the project that owns the Cloud Source Repository.
If omitted, the project ID requesting the build is assumed.</rdfs:comment>
    <rdfs:domain rdf:resource="http://example.org/onto/class/google_cloudbuild_trigger"/>
    <rdfs:range rdf:resource="http://www.w3.org/2001/XMLSchema#string"/>
  </owl:DatatypeProperty>
  <owl:DatatypeProperty rdf:about="http://example.org/onto/prop/google_cloudbuild_trigger_repo_name">
    <rdfs:label>repo_name</rdfs:label>
    <rdfs:comment>Name of the Cloud Source Repository.</rdfs:comment>
    <rdfs:domain rdf:resource="http://example.org/onto/class/google_cloudbuild_trigger"/>
    <rdfs:range rdf:resource="http://www.w3.org/2001/XMLSchema#string"/>
  </owl:DatatypeProperty>
  <owl:DatatypeProperty rdf:about="http://example.org/onto/prop/google_cloudbuild_trigger_substitutions">
    <rdfs:label>substitutions</rdfs:label>
    <rdfs:comment>Substitutions to use in a triggered build. Should only be used with triggers.run</rdfs:comment>
    <rdfs:domain rdf:resource="http://example.org/onto/class/google_cloudbuild_trigger"/>
    <rdfs:range rdf:resource="http://www.w3.org/2001/XMLSchema#string"/>
  </owl:DatatypeProperty>
  <owl:DatatypeProperty rdf:about="http://example.org/onto/prop/google_cloudbuild_trigger_tag_name">
    <rdfs:label>tag_name</rdfs:label>
    <rdfs:comment>Regex matching tags to build. Exactly one a of branch name, tag, or commit SHA must be provided.
The syntax of the regular expressions accepted is the syntax accepted by RE2 and
described at https://github.com/google/re2/wiki/Syntax</rdfs:comment>
    <rdfs:domain rdf:resource="http://example.org/onto/class/google_cloudbuild_trigger"/>
    <rdfs:range rdf:resource="http://www.w3.org/2001/XMLSchema#string"/>
  </owl:DatatypeProperty>
  <owl:DatatypeProperty rdf:about="http://example.org/onto/prop/google_cloudbuild_trigger_bucket">
    <rdfs:label>bucket</rdfs:label>
    <rdfs:comment>Google Cloud Storage bucket containing the source.</rdfs:comment>
    <rdfs:domain rdf:resource="http://example.org/onto/class/google_cloudbuild_trigger"/>
    <rdfs:range rdf:resource="http://www.w3.org/2001/XMLSchema#string"/>
  </owl:DatatypeProperty>
  <owl:DatatypeProperty rdf:about="http://example.org/onto/prop/google_cloudbuild_trigger_generation">
    <rdfs:label>generation</rdfs:label>
    <rdfs:comment>Google Cloud Storage generation for the object.
If the generation is omitted, the latest generation will be used</rdfs:comment>
    <rdfs:domain rdf:resource="http://example.org/onto/class/google_cloudbuild_trigger"/>
    <rdfs:range rdf:resource="http://www.w3.org/2001/XMLSchema#string"/>
  </owl:DatatypeProperty>
  <owl:DatatypeProperty rdf:about="http://example.org/onto/prop/google_cloudbuild_trigger_object">
    <rdfs:label>object</rdfs:label>
    <rdfs:comment>Google Cloud Storage object containing the source.
This object must be a gzipped archive file (.tar.gz) containing source to build.</rdfs:comment>
    <rdfs:domain rdf:resource="http://example.org/onto/class/google_cloudbuild_trigger"/>
    <rdfs:range rdf:resource="http://www.w3.org/2001/XMLSchema#string"/>
  </owl:DatatypeProperty>
  <owl:DatatypeProperty rdf:about="http://example.org/onto/prop/google_cloudbuild_trigger_allow_exit_codes">
    <rdfs:label>allow_exit_codes</rdfs:label>
    <rdfs:comment>Allow this build step to fail without failing the entire build if and
only if the exit code is one of the specified codes.

If 'allowFailure' is also specified, this field will take precedence.</rdfs:comment>
    <rdfs:domain rdf:resource="http://example.org/onto/class/google_cloudbuild_trigger"/>
    <rdfs:range rdf:resource="http://www.w3.org/2001/XMLSchema#string"/>
  </owl:DatatypeProperty>
  <owl:DatatypeProperty rdf:about="http://example.org/onto/prop/google_cloudbuild_trigger_allow_failure">
    <rdfs:label>allow_failure</rdfs:label>
    <rdfs:comment>Allow this build step to fail without failing the entire build.
If false, the entire build will fail if this step fails. Otherwise, the
build will succeed, but this step will still have a failure status.
Error information will be reported in the 'failureDetail' field.

'allowExitCodes' takes precedence over this field.</rdfs:comment>
    <rdfs:domain rdf:resource="http://example.org/onto/class/google_cloudbuild_trigger"/>
    <rdfs:range rdf:resource="http://www.w3.org/2001/XMLSchema#string"/>
  </owl:DatatypeProperty>
  <owl:DatatypeProperty rdf:about="http://example.org/onto/prop/google_cloudbuild_trigger_args">
    <rdfs:label>args</rdfs:label>
    <rdfs:comment>A list of arguments that will be presented to the step when it is started.

If the image used to run the step's container has an entrypoint, the args
are used as arguments to that entrypoint. If the image does not define an
entrypoint, the first element in args is used as the entrypoint, and the
remainder will be used as arguments.</rdfs:comment>
    <rdfs:domain rdf:resource="http://example.org/onto/class/google_cloudbuild_trigger"/>
    <rdfs:range rdf:resource="http://www.w3.org/2001/XMLSchema#string"/>
  </owl:DatatypeProperty>
  <owl:DatatypeProperty rdf:about="http://example.org/onto/prop/google_cloudbuild_trigger_dir">
    <rdfs:label>dir</rdfs:label>
    <rdfs:comment>Working directory to use when running this step's container.

If this value is a relative path, it is relative to the build's working
directory. If this value is absolute, it may be outside the build's working
directory, in which case the contents of the path may not be persisted
across build step executions, unless a 'volume' for that path is specified.

If the build specifies a 'RepoSource' with 'dir' and a step with a
'dir',
which specifies an absolute path, the 'RepoSource' 'dir' is ignored
for the step's execution.</rdfs:comment>
    <rdfs:domain rdf:resource="http://example.org/onto/class/google_cloudbuild_trigger"/>
    <rdfs:range rdf:resource="http://www.w3.org/2001/XMLSchema#string"/>
  </owl:DatatypeProperty>
  <owl:DatatypeProperty rdf:about="http://example.org/onto/prop/google_cloudbuild_trigger_entrypoint">
    <rdfs:label>entrypoint</rdfs:label>
    <rdfs:comment>Entrypoint to be used instead of the build step image's
default entrypoint.
If unset, the image's default entrypoint is used</rdfs:comment>
    <rdfs:domain rdf:resource="http://example.org/onto/class/google_cloudbuild_trigger"/>
    <rdfs:range rdf:resource="http://www.w3.org/2001/XMLSchema#string"/>
  </owl:DatatypeProperty>
  <owl:DatatypeProperty rdf:about="http://example.org/onto/prop/google_cloudbuild_trigger_env">
    <rdfs:label>env</rdfs:label>
    <rdfs:comment>A list of environment variable definitions to be used when
running a step.

The elements are of the form "KEY=VALUE" for the environment variable
"KEY" being given the value "VALUE".</rdfs:comment>
    <rdfs:domain rdf:resource="http://example.org/onto/class/google_cloudbuild_trigger"/>
    <rdfs:range rdf:resource="http://www.w3.org/2001/XMLSchema#string"/>
  </owl:DatatypeProperty>
  <owl:DatatypeProperty rdf:about="http://example.org/onto/prop/google_cloudbuild_trigger_id">
    <rdfs:label>id</rdfs:label>
    <rdfs:comment>Unique identifier for this build step, used in 'wait_for' to
reference this build step as a dependency.</rdfs:comment>
    <rdfs:domain rdf:resource="http://example.org/onto/class/google_cloudbuild_trigger"/>
    <rdfs:range rdf:resource="http://www.w3.org/2001/XMLSchema#string"/>
  </owl:DatatypeProperty>
  <owl:DatatypeProperty rdf:about="http://example.org/onto/prop/google_cloudbuild_trigger_name">
    <rdfs:label>name</rdfs:label>
    <rdfs:comment>The name of the container image that will run this particular build step.

If the image is available in the host's Docker daemon's cache, it will be
run directly. If not, the host will attempt to pull the image first, using
the builder service account's credentials if necessary.

The Docker daemon's cache will already have the latest versions of all of
the officially supported build steps (see https://github.com/GoogleCloudPlatform/cloud-builders
for images and examples).
The Docker daemon will also have cached many of the layers for some popular
images, like "ubuntu", "debian", but they will be refreshed at the time
you attempt to use them.

If you built an image in a previous build step, it will be stored in the
host's Docker daemon's cache and is available to use as the name for a
later build step.</rdfs:comment>
    <rdfs:domain rdf:resource="http://example.org/onto/class/google_cloudbuild_trigger"/>
    <rdfs:range rdf:resource="http://www.w3.org/2001/XMLSchema#string"/>
  </owl:DatatypeProperty>
  <owl:DatatypeProperty rdf:about="http://example.org/onto/prop/google_cloudbuild_trigger_script">
    <rdfs:label>script</rdfs:label>
    <rdfs:comment>A shell script to be executed in the step.
When script is provided, the user cannot specify the entrypoint or args.</rdfs:comment>
    <rdfs:domain rdf:resource="http://example.org/onto/class/google_cloudbuild_trigger"/>
    <rdfs:range rdf:resource="http://www.w3.org/2001/XMLSchema#string"/>
  </owl:DatatypeProperty>
  <owl:DatatypeProperty rdf:about="http://example.org/onto/prop/google_cloudbuild_trigger_secret_env">
    <rdfs:label>secret_env</rdfs:label>
    <rdfs:comment>A list of environment variables which are encrypted using
a Cloud Key
Management Service crypto key. These values must be specified in
the build's 'Secret'.</rdfs:comment>
    <rdfs:domain rdf:resource="http://example.org/onto/class/google_cloudbuild_trigger"/>
    <rdfs:range rdf:resource="http://www.w3.org/2001/XMLSchema#string"/>
  </owl:DatatypeProperty>
  <owl:DatatypeProperty rdf:about="http://example.org/onto/prop/google_cloudbuild_trigger_timeout">
    <rdfs:label>timeout</rdfs:label>
    <rdfs:comment>Time limit for executing this build step. If not defined,
the step has no
time limit and will be allowed to continue to run until either it
completes or the build itself times out.</rdfs:comment>
    <rdfs:domain rdf:resource="http://example.org/onto/class/google_cloudbuild_trigger"/>
    <rdfs:range rdf:resource="http://www.w3.org/2001/XMLSchema#string"/>
  </owl:DatatypeProperty>
  <owl:DatatypeProperty rdf:about="http://example.org/onto/prop/google_cloudbuild_trigger_timing">
    <rdfs:label>timing</rdfs:label>
    <rdfs:comment>Output only. Stores timing information for executing this
build step.</rdfs:comment>
    <rdfs:domain rdf:resource="http://example.org/onto/class/google_cloudbuild_trigger"/>
    <rdfs:range rdf:resource="http://www.w3.org/2001/XMLSchema#string"/>
  </owl:DatatypeProperty>
  <owl:DatatypeProperty rdf:about="http://example.org/onto/prop/google_cloudbuild_trigger_wait_for">
    <rdfs:label>wait_for</rdfs:label>
    <rdfs:comment>The ID(s) of the step(s) that this build step depends on.

This build step will not start until all the build steps in 'wait_for'
have completed successfully. If 'wait_for' is empty, this build step
will start when all previous build steps in the 'Build.Steps' list
have completed successfully.</rdfs:comment>
    <rdfs:domain rdf:resource="http://example.org/onto/class/google_cloudbuild_trigger"/>
    <rdfs:range rdf:resource="http://www.w3.org/2001/XMLSchema#string"/>
  </owl:DatatypeProperty>
  <owl:DatatypeProperty rdf:about="http://example.org/onto/prop/google_cloudbuild_trigger_name">
    <rdfs:label>name</rdfs:label>
    <rdfs:comment>Name of the volume to mount.

Volume names must be unique per build step and must be valid names for
Docker volumes. Each named volume must be used by at least two build steps.</rdfs:comment>
    <rdfs:domain rdf:resource="http://example.org/onto/class/google_cloudbuild_trigger"/>
    <rdfs:range rdf:resource="http://www.w3.org/2001/XMLSchema#string"/>
  </owl:DatatypeProperty>
  <owl:DatatypeProperty rdf:about="http://example.org/onto/prop/google_cloudbuild_trigger_path">
    <rdfs:label>path</rdfs:label>
    <rdfs:comment>Path at which to mount the volume.

Paths must be absolute and cannot conflict with other volume paths on
the same build step or with certain reserved volume paths.</rdfs:comment>
    <rdfs:domain rdf:resource="http://example.org/onto/class/google_cloudbuild_trigger"/>
    <rdfs:range rdf:resource="http://www.w3.org/2001/XMLSchema#string"/>
  </owl:DatatypeProperty>
  <owl:DatatypeProperty rdf:about="http://example.org/onto/prop/google_cloudbuild_trigger_git_repository_link">
    <rdfs:label>git_repository_link</rdfs:label>
    <rdfs:comment>The Developer Connect Git repository link, formatted as 'projects/*/locations/*/connections/*/gitRepositoryLink/*'.</rdfs:comment>
    <rdfs:domain rdf:resource="http://example.org/onto/class/google_cloudbuild_trigger"/>
    <rdfs:range rdf:resource="http://www.w3.org/2001/XMLSchema#string"/>
  </owl:DatatypeProperty>
  <owl:DatatypeProperty rdf:about="http://example.org/onto/prop/google_cloudbuild_trigger_git_repository_link_type">
    <rdfs:label>git_repository_link_type</rdfs:label>
    <rdfs:comment>The type of DeveloperConnect GitRepositoryLink.</rdfs:comment>
    <rdfs:domain rdf:resource="http://example.org/onto/class/google_cloudbuild_trigger"/>
    <rdfs:range rdf:resource="http://www.w3.org/2001/XMLSchema#string"/>
  </owl:DatatypeProperty>
  <owl:DatatypeProperty rdf:about="http://example.org/onto/prop/google_cloudbuild_trigger_branch">
    <rdfs:label>branch</rdfs:label>
    <rdfs:comment>Regex of branches to match.</rdfs:comment>
    <rdfs:domain rdf:resource="http://example.org/onto/class/google_cloudbuild_trigger"/>
    <rdfs:range rdf:resource="http://www.w3.org/2001/XMLSchema#string"/>
  </owl:DatatypeProperty>
  <owl:DatatypeProperty rdf:about="http://example.org/onto/prop/google_cloudbuild_trigger_comment_control">
    <rdfs:label>comment_control</rdfs:label>
    <rdfs:comment>Configure builds to run whether a repository owner or collaborator need to comment '/gcbrun'. Possible values: ["COMMENTS_DISABLED", "COMMENTS_ENABLED", "COMMENTS_ENABLED_FOR_EXTERNAL_CONTRIBUTORS_ONLY"]</rdfs:comment>
    <rdfs:domain rdf:resource="http://example.org/onto/class/google_cloudbuild_trigger"/>
    <rdfs:range rdf:resource="http://www.w3.org/2001/XMLSchema#string"/>
  </owl:DatatypeProperty>
  <owl:DatatypeProperty rdf:about="http://example.org/onto/prop/google_cloudbuild_trigger_invert_regex">
    <rdfs:label>invert_regex</rdfs:label>
    <rdfs:comment>If true, branches that do NOT match the git_ref will trigger a build.</rdfs:comment>
    <rdfs:domain rdf:resource="http://example.org/onto/class/google_cloudbuild_trigger"/>
    <rdfs:range rdf:resource="http://www.w3.org/2001/XMLSchema#string"/>
  </owl:DatatypeProperty>
  <owl:DatatypeProperty rdf:about="http://example.org/onto/prop/google_cloudbuild_trigger_branch">
    <rdfs:label>branch</rdfs:label>
    <rdfs:comment>Regex of branches to match.</rdfs:comment>
    <rdfs:domain rdf:resource="http://example.org/onto/class/google_cloudbuild_trigger"/>
    <rdfs:range rdf:resource="http://www.w3.org/2001/XMLSchema#string"/>
  </owl:DatatypeProperty>
  <owl:DatatypeProperty rdf:about="http://example.org/onto/prop/google_cloudbuild_trigger_invert_regex">
    <rdfs:label>invert_regex</rdfs:label>
    <rdfs:comment>If true, only trigger a build if the revision regex does NOT match the git_ref regex.</rdfs:comment>
    <rdfs:domain rdf:resource="http://example.org/onto/class/google_cloudbuild_trigger"/>
    <rdfs:range rdf:resource="http://www.w3.org/2001/XMLSchema#string"/>
  </owl:DatatypeProperty>
  <owl:DatatypeProperty rdf:about="http://example.org/onto/prop/google_cloudbuild_trigger_tag">
    <rdfs:label>tag</rdfs:label>
    <rdfs:comment>Regex of tags to match.</rdfs:comment>
    <rdfs:domain rdf:resource="http://example.org/onto/class/google_cloudbuild_trigger"/>
    <rdfs:range rdf:resource="http://www.w3.org/2001/XMLSchema#string"/>
  </owl:DatatypeProperty>
  <owl:DatatypeProperty rdf:about="http://example.org/onto/prop/google_cloudbuild_trigger_bitbucket_server_config">
    <rdfs:label>bitbucket_server_config</rdfs:label>
    <rdfs:comment>The full resource name of the bitbucket server config.
Format: projects/{project}/locations/{location}/bitbucketServerConfigs/{id}.</rdfs:comment>
    <rdfs:domain rdf:resource="http://example.org/onto/class/google_cloudbuild_trigger"/>
    <rdfs:range rdf:resource="http://www.w3.org/2001/XMLSchema#string"/>
  </owl:DatatypeProperty>
  <owl:DatatypeProperty rdf:about="http://example.org/onto/prop/google_cloudbuild_trigger_github_enterprise_config">
    <rdfs:label>github_enterprise_config</rdfs:label>
    <rdfs:comment>The full resource name of the github enterprise config.
Format: projects/{project}/locations/{location}/githubEnterpriseConfigs/{id}. projects/{project}/githubEnterpriseConfigs/{id}.</rdfs:comment>
    <rdfs:domain rdf:resource="http://example.org/onto/class/google_cloudbuild_trigger"/>
    <rdfs:range rdf:resource="http://www.w3.org/2001/XMLSchema#string"/>
  </owl:DatatypeProperty>
  <owl:DatatypeProperty rdf:about="http://example.org/onto/prop/google_cloudbuild_trigger_path">
    <rdfs:label>path</rdfs:label>
    <rdfs:comment>The path of the file, with the repo root as the root of the path.</rdfs:comment>
    <rdfs:domain rdf:resource="http://example.org/onto/class/google_cloudbuild_trigger"/>
    <rdfs:range rdf:resource="http://www.w3.org/2001/XMLSchema#string"/>
  </owl:DatatypeProperty>
  <owl:DatatypeProperty rdf:about="http://example.org/onto/prop/google_cloudbuild_trigger_repo_type">
    <rdfs:label>repo_type</rdfs:label>
    <rdfs:comment>The type of the repo, since it may not be explicit from the repo field (e.g from a URL).
Values can be UNKNOWN, CLOUD_SOURCE_REPOSITORIES, GITHUB, BITBUCKET_SERVER Possible values: ["UNKNOWN", "CLOUD_SOURCE_REPOSITORIES", "GITHUB", "BITBUCKET_SERVER"]</rdfs:comment>
    <rdfs:domain rdf:resource="http://example.org/onto/class/google_cloudbuild_trigger"/>
    <rdfs:range rdf:resource="http://www.w3.org/2001/XMLSchema#string"/>
  </owl:DatatypeProperty>
  <owl:DatatypeProperty rdf:about="http://example.org/onto/prop/google_cloudbuild_trigger_repository">
    <rdfs:label>repository</rdfs:label>
    <rdfs:comment>The fully qualified resource name of the Repo API repository. The fully qualified resource name of the Repo API repository.
If unspecified, the repo from which the trigger invocation originated is assumed to be the repo from which to read the specified path.</rdfs:comment>
    <rdfs:domain rdf:resource="http://example.org/onto/class/google_cloudbuild_trigger"/>
    <rdfs:range rdf:resource="http://www.w3.org/2001/XMLSchema#string"/>
  </owl:DatatypeProperty>
  <owl:DatatypeProperty rdf:about="http://example.org/onto/prop/google_cloudbuild_trigger_revision">
    <rdfs:label>revision</rdfs:label>
    <rdfs:comment>The branch, tag, arbitrary ref, or SHA version of the repo to use when resolving the
filename (optional). This field respects the same syntax/resolution as described here: https://git-scm.com/docs/gitrevisions
If unspecified, the revision from which the trigger invocation originated is assumed to be the revision from which to read the specified path.</rdfs:comment>
    <rdfs:domain rdf:resource="http://example.org/onto/class/google_cloudbuild_trigger"/>
    <rdfs:range rdf:resource="http://www.w3.org/2001/XMLSchema#string"/>
  </owl:DatatypeProperty>
  <owl:DatatypeProperty rdf:about="http://example.org/onto/prop/google_cloudbuild_trigger_uri">
    <rdfs:label>uri</rdfs:label>
    <rdfs:comment>The URI of the repo (optional). If unspecified, the repo from which the trigger
invocation originated is assumed to be the repo from which to read the specified path.</rdfs:comment>
    <rdfs:domain rdf:resource="http://example.org/onto/class/google_cloudbuild_trigger"/>
    <rdfs:range rdf:resource="http://www.w3.org/2001/XMLSchema#string"/>
  </owl:DatatypeProperty>
  <owl:DatatypeProperty rdf:about="http://example.org/onto/prop/google_cloudbuild_trigger_enterprise_config_resource_name">
    <rdfs:label>enterprise_config_resource_name</rdfs:label>
    <rdfs:comment>The resource name of the github enterprise config that should be applied to this installation.
For example: "projects/{$projectId}/locations/{$locationId}/githubEnterpriseConfigs/{$configId}"</rdfs:comment>
    <rdfs:domain rdf:resource="http://example.org/onto/class/google_cloudbuild_trigger"/>
    <rdfs:range rdf:resource="http://www.w3.org/2001/XMLSchema#string"/>
  </owl:DatatypeProperty>
  <owl:DatatypeProperty rdf:about="http://example.org/onto/prop/google_cloudbuild_trigger_name">
    <rdfs:label>name</rdfs:label>
    <rdfs:comment>Name of the repository. For example: The name for
https://github.com/googlecloudplatform/cloud-builders is "cloud-builders".</rdfs:comment>
    <rdfs:domain rdf:resource="http://example.org/onto/class/google_cloudbuild_trigger"/>
    <rdfs:range rdf:resource="http://www.w3.org/2001/XMLSchema#string"/>
  </owl:DatatypeProperty>
  <owl:DatatypeProperty rdf:about="http://example.org/onto/prop/google_cloudbuild_trigger_owner">
    <rdfs:label>owner</rdfs:label>
    <rdfs:comment>Owner of the repository. For example: The owner for
https://github.com/googlecloudplatform/cloud-builders is "googlecloudplatform".</rdfs:comment>
    <rdfs:domain rdf:resource="http://example.org/onto/class/google_cloudbuild_trigger"/>
    <rdfs:range rdf:resource="http://www.w3.org/2001/XMLSchema#string"/>
  </owl:DatatypeProperty>
  <owl:DatatypeProperty rdf:about="http://example.org/onto/prop/google_cloudbuild_trigger_branch">
    <rdfs:label>branch</rdfs:label>
    <rdfs:comment>Regex of branches to match.</rdfs:comment>
    <rdfs:domain rdf:resource="http://example.org/onto/class/google_cloudbuild_trigger"/>
    <rdfs:range rdf:resource="http://www.w3.org/2001/XMLSchema#string"/>
  </owl:DatatypeProperty>
  <owl:DatatypeProperty rdf:about="http://example.org/onto/prop/google_cloudbuild_trigger_comment_control">
    <rdfs:label>comment_control</rdfs:label>
    <rdfs:comment>Whether to block builds on a "/gcbrun" comment from a repository owner or collaborator. Possible values: ["COMMENTS_DISABLED", "COMMENTS_ENABLED", "COMMENTS_ENABLED_FOR_EXTERNAL_CONTRIBUTORS_ONLY"]</rdfs:comment>
    <rdfs:domain rdf:resource="http://example.org/onto/class/google_cloudbuild_trigger"/>
    <rdfs:range rdf:resource="http://www.w3.org/2001/XMLSchema#string"/>
  </owl:DatatypeProperty>
  <owl:DatatypeProperty rdf:about="http://example.org/onto/prop/google_cloudbuild_trigger_invert_regex">
    <rdfs:label>invert_regex</rdfs:label>
    <rdfs:comment>If true, branches that do NOT match the git_ref will trigger a build.</rdfs:comment>
    <rdfs:domain rdf:resource="http://example.org/onto/class/google_cloudbuild_trigger"/>
    <rdfs:range rdf:resource="http://www.w3.org/2001/XMLSchema#string"/>
  </owl:DatatypeProperty>
  <owl:DatatypeProperty rdf:about="http://example.org/onto/prop/google_cloudbuild_trigger_branch">
    <rdfs:label>branch</rdfs:label>
    <rdfs:comment>Regex of branches to match.  Specify only one of branch or tag.</rdfs:comment>
    <rdfs:domain rdf:resource="http://example.org/onto/class/google_cloudbuild_trigger"/>
    <rdfs:range rdf:resource="http://www.w3.org/2001/XMLSchema#string"/>
  </owl:DatatypeProperty>
  <owl:DatatypeProperty rdf:about="http://example.org/onto/prop/google_cloudbuild_trigger_invert_regex">
    <rdfs:label>invert_regex</rdfs:label>
    <rdfs:comment>When true, only trigger a build if the revision regex does NOT match the git_ref regex.</rdfs:comment>
    <rdfs:domain rdf:resource="http://example.org/onto/class/google_cloudbuild_trigger"/>
    <rdfs:range rdf:resource="http://www.w3.org/2001/XMLSchema#string"/>
  </owl:DatatypeProperty>
  <owl:DatatypeProperty rdf:about="http://example.org/onto/prop/google_cloudbuild_trigger_tag">
    <rdfs:label>tag</rdfs:label>
    <rdfs:comment>Regex of tags to match.  Specify only one of branch or tag.</rdfs:comment>
    <rdfs:domain rdf:resource="http://example.org/onto/class/google_cloudbuild_trigger"/>
    <rdfs:range rdf:resource="http://www.w3.org/2001/XMLSchema#string"/>
  </owl:DatatypeProperty>
  <owl:DatatypeProperty rdf:about="http://example.org/onto/prop/google_cloudbuild_trigger_service_account_email">
    <rdfs:label>service_account_email</rdfs:label>
    <rdfs:comment>Service account that will make the push request.</rdfs:comment>
    <rdfs:domain rdf:resource="http://example.org/onto/class/google_cloudbuild_trigger"/>
    <rdfs:range rdf:resource="http://www.w3.org/2001/XMLSchema#string"/>
  </owl:DatatypeProperty>
  <owl:DatatypeProperty rdf:about="http://example.org/onto/prop/google_cloudbuild_trigger_state">
    <rdfs:label>state</rdfs:label>
    <rdfs:comment>Potential issues with the underlying Pub/Sub subscription configuration.
Only populated on get requests.</rdfs:comment>
    <rdfs:domain rdf:resource="http://example.org/onto/class/google_cloudbuild_trigger"/>
    <rdfs:range rdf:resource="http://www.w3.org/2001/XMLSchema#string"/>
  </owl:DatatypeProperty>
  <owl:DatatypeProperty rdf:about="http://example.org/onto/prop/google_cloudbuild_trigger_subscription">
    <rdfs:label>subscription</rdfs:label>
    <rdfs:comment>Output only. Name of the subscription.</rdfs:comment>
    <rdfs:domain rdf:resource="http://example.org/onto/class/google_cloudbuild_trigger"/>
    <rdfs:range rdf:resource="http://www.w3.org/2001/XMLSchema#string"/>
  </owl:DatatypeProperty>
  <owl:DatatypeProperty rdf:about="http://example.org/onto/prop/google_cloudbuild_trigger_topic">
    <rdfs:label>topic</rdfs:label>
    <rdfs:comment>The name of the topic from which this subscription is receiving messages.</rdfs:comment>
    <rdfs:domain rdf:resource="http://example.org/onto/class/google_cloudbuild_trigger"/>
    <rdfs:range rdf:resource="http://www.w3.org/2001/XMLSchema#string"/>
  </owl:DatatypeProperty>
  <owl:DatatypeProperty rdf:about="http://example.org/onto/prop/google_cloudbuild_trigger_repository">
    <rdfs:label>repository</rdfs:label>
    <rdfs:comment>The resource name of the Repo API resource.</rdfs:comment>
    <rdfs:domain rdf:resource="http://example.org/onto/class/google_cloudbuild_trigger"/>
    <rdfs:range rdf:resource="http://www.w3.org/2001/XMLSchema#string"/>
  </owl:DatatypeProperty>
  <owl:DatatypeProperty rdf:about="http://example.org/onto/prop/google_cloudbuild_trigger_branch">
    <rdfs:label>branch</rdfs:label>
    <rdfs:comment>Regex of branches to match.

The syntax of the regular expressions accepted is the syntax accepted by
RE2 and described at https://github.com/google/re2/wiki/Syntax</rdfs:comment>
    <rdfs:domain rdf:resource="http://example.org/onto/class/google_cloudbuild_trigger"/>
    <rdfs:range rdf:resource="http://www.w3.org/2001/XMLSchema#string"/>
  </owl:DatatypeProperty>
  <owl:DatatypeProperty rdf:about="http://example.org/onto/prop/google_cloudbuild_trigger_comment_control">
    <rdfs:label>comment_control</rdfs:label>
    <rdfs:comment>Configure builds to run whether a repository owner or collaborator need to comment '/gcbrun'. Possible values: ["COMMENTS_DISABLED", "COMMENTS_ENABLED", "COMMENTS_ENABLED_FOR_EXTERNAL_CONTRIBUTORS_ONLY"]</rdfs:comment>
    <rdfs:domain rdf:resource="http://example.org/onto/class/google_cloudbuild_trigger"/>
    <rdfs:range rdf:resource="http://www.w3.org/2001/XMLSchema#string"/>
  </owl:DatatypeProperty>
  <owl:DatatypeProperty rdf:about="http://example.org/onto/prop/google_cloudbuild_trigger_invert_regex">
    <rdfs:label>invert_regex</rdfs:label>
    <rdfs:comment>If true, branches that do NOT match the git_ref will trigger a build.</rdfs:comment>
    <rdfs:domain rdf:resource="http://example.org/onto/class/google_cloudbuild_trigger"/>
    <rdfs:range rdf:resource="http://www.w3.org/2001/XMLSchema#string"/>
  </owl:DatatypeProperty>
  <owl:DatatypeProperty rdf:about="http://example.org/onto/prop/google_cloudbuild_trigger_branch">
    <rdfs:label>branch</rdfs:label>
    <rdfs:comment>Regex of branches to match.

The syntax of the regular expressions accepted is the syntax accepted by
RE2 and described at https://github.com/google/re2/wiki/Syntax</rdfs:comment>
    <rdfs:domain rdf:resource="http://example.org/onto/class/google_cloudbuild_trigger"/>
    <rdfs:range rdf:resource="http://www.w3.org/2001/XMLSchema#string"/>
  </owl:DatatypeProperty>
  <owl:DatatypeProperty rdf:about="http://example.org/onto/prop/google_cloudbuild_trigger_invert_regex">
    <rdfs:label>invert_regex</rdfs:label>
    <rdfs:comment>If true, only trigger a build if the revision regex does NOT match the git_ref regex.</rdfs:comment>
    <rdfs:domain rdf:resource="http://example.org/onto/class/google_cloudbuild_trigger"/>
    <rdfs:range rdf:resource="http://www.w3.org/2001/XMLSchema#string"/>
  </owl:DatatypeProperty>
  <owl:DatatypeProperty rdf:about="http://example.org/onto/prop/google_cloudbuild_trigger_tag">
    <rdfs:label>tag</rdfs:label>
    <rdfs:comment>Regex of tags to match.

The syntax of the regular expressions accepted is the syntax accepted by
RE2 and described at https://github.com/google/re2/wiki/Syntax</rdfs:comment>
    <rdfs:domain rdf:resource="http://example.org/onto/class/google_cloudbuild_trigger"/>
    <rdfs:range rdf:resource="http://www.w3.org/2001/XMLSchema#string"/>
  </owl:DatatypeProperty>
  <owl:DatatypeProperty rdf:about="http://example.org/onto/prop/google_cloudbuild_trigger_bitbucket_server_config">
    <rdfs:label>bitbucket_server_config</rdfs:label>
    <rdfs:comment>The full resource name of the bitbucket server config.
Format: projects/{project}/locations/{location}/bitbucketServerConfigs/{id}.</rdfs:comment>
    <rdfs:domain rdf:resource="http://example.org/onto/class/google_cloudbuild_trigger"/>
    <rdfs:range rdf:resource="http://www.w3.org/2001/XMLSchema#string"/>
  </owl:DatatypeProperty>
  <owl:DatatypeProperty rdf:about="http://example.org/onto/prop/google_cloudbuild_trigger_github_enterprise_config">
    <rdfs:label>github_enterprise_config</rdfs:label>
    <rdfs:comment>The full resource name of the github enterprise config.
Format: projects/{project}/locations/{location}/githubEnterpriseConfigs/{id}. projects/{project}/githubEnterpriseConfigs/{id}.</rdfs:comment>
    <rdfs:domain rdf:resource="http://example.org/onto/class/google_cloudbuild_trigger"/>
    <rdfs:range rdf:resource="http://www.w3.org/2001/XMLSchema#string"/>
  </owl:DatatypeProperty>
  <owl:DatatypeProperty rdf:about="http://example.org/onto/prop/google_cloudbuild_trigger_ref">
    <rdfs:label>ref</rdfs:label>
    <rdfs:comment>The branch or tag to use. Must start with "refs/" (required).</rdfs:comment>
    <rdfs:domain rdf:resource="http://example.org/onto/class/google_cloudbuild_trigger"/>
    <rdfs:range rdf:resource="http://www.w3.org/2001/XMLSchema#string"/>
  </owl:DatatypeProperty>
  <owl:DatatypeProperty rdf:about="http://example.org/onto/prop/google_cloudbuild_trigger_repo_type">
    <rdfs:label>repo_type</rdfs:label>
    <rdfs:comment>The type of the repo, since it may not be explicit from the repo field (e.g from a URL).
Values can be UNKNOWN, CLOUD_SOURCE_REPOSITORIES, GITHUB, BITBUCKET_SERVER Possible values: ["UNKNOWN", "CLOUD_SOURCE_REPOSITORIES", "GITHUB", "BITBUCKET_SERVER"]</rdfs:comment>
    <rdfs:domain rdf:resource="http://example.org/onto/class/google_cloudbuild_trigger"/>
    <rdfs:range rdf:resource="http://www.w3.org/2001/XMLSchema#string"/>
  </owl:DatatypeProperty>
  <owl:DatatypeProperty rdf:about="http://example.org/onto/prop/google_cloudbuild_trigger_repository">
    <rdfs:label>repository</rdfs:label>
    <rdfs:comment>The qualified resource name of the Repo API repository.
Either uri or repository can be specified and is required.</rdfs:comment>
    <rdfs:domain rdf:resource="http://example.org/onto/class/google_cloudbuild_trigger"/>
    <rdfs:range rdf:resource="http://www.w3.org/2001/XMLSchema#string"/>
  </owl:DatatypeProperty>
  <owl:DatatypeProperty rdf:about="http://example.org/onto/prop/google_cloudbuild_trigger_uri">
    <rdfs:label>uri</rdfs:label>
    <rdfs:comment>The URI of the repo.</rdfs:comment>
    <rdfs:domain rdf:resource="http://example.org/onto/class/google_cloudbuild_trigger"/>
    <rdfs:range rdf:resource="http://www.w3.org/2001/XMLSchema#string"/>
  </owl:DatatypeProperty>
  <owl:DatatypeProperty rdf:about="http://example.org/onto/prop/google_cloudbuild_trigger_create">
    <rdfs:label>create</rdfs:label>
    <rdfs:domain rdf:resource="http://example.org/onto/class/google_cloudbuild_trigger"/>
    <rdfs:range rdf:resource="http://www.w3.org/2001/XMLSchema#string"/>
  </owl:DatatypeProperty>
  <owl:DatatypeProperty rdf:about="http://example.org/onto/prop/google_cloudbuild_trigger_delete">
    <rdfs:label>delete</rdfs:label>
    <rdfs:domain rdf:resource="http://example.org/onto/class/google_cloudbuild_trigger"/>
    <rdfs:range rdf:resource="http://www.w3.org/2001/XMLSchema#string"/>
  </owl:DatatypeProperty>
  <owl:DatatypeProperty rdf:about="http://example.org/onto/prop/google_cloudbuild_trigger_update">
    <rdfs:label>update</rdfs:label>
    <rdfs:domain rdf:resource="http://example.org/onto/class/google_cloudbuild_trigger"/>
    <rdfs:range rdf:resource="http://www.w3.org/2001/XMLSchema#string"/>
  </owl:DatatypeProperty>
  <owl:DatatypeProperty rdf:about="http://example.org/onto/prop/google_cloudbuild_trigger_branch_name">
    <rdfs:label>branch_name</rdfs:label>
    <rdfs:comment>Name of the branch to build. Exactly one a of branch name, tag, or commit SHA must be provided.
This field is a regular expression.</rdfs:comment>
    <rdfs:domain rdf:resource="http://example.org/onto/class/google_cloudbuild_trigger"/>
    <rdfs:range rdf:resource="http://www.w3.org/2001/XMLSchema#string"/>
  </owl:DatatypeProperty>
  <owl:DatatypeProperty rdf:about="http://example.org/onto/prop/google_cloudbuild_trigger_commit_sha">
    <rdfs:label>commit_sha</rdfs:label>
    <rdfs:comment>Explicit commit SHA to build. Exactly one of a branch name, tag, or commit SHA must be provided.</rdfs:comment>
    <rdfs:domain rdf:resource="http://example.org/onto/class/google_cloudbuild_trigger"/>
    <rdfs:range rdf:resource="http://www.w3.org/2001/XMLSchema#string"/>
  </owl:DatatypeProperty>
  <owl:DatatypeProperty rdf:about="http://example.org/onto/prop/google_cloudbuild_trigger_dir">
    <rdfs:label>dir</rdfs:label>
    <rdfs:comment>Directory, relative to the source root, in which to run the build.

This must be a relative path. If a step's dir is specified and
is an absolute path, this value is ignored for that step's
execution.</rdfs:comment>
    <rdfs:domain rdf:resource="http://example.org/onto/class/google_cloudbuild_trigger"/>
    <rdfs:range rdf:resource="http://www.w3.org/2001/XMLSchema#string"/>
  </owl:DatatypeProperty>
  <owl:DatatypeProperty rdf:about="http://example.org/onto/prop/google_cloudbuild_trigger_invert_regex">
    <rdfs:label>invert_regex</rdfs:label>
    <rdfs:comment>Only trigger a build if the revision regex does NOT match the revision regex.</rdfs:comment>
    <rdfs:domain rdf:resource="http://example.org/onto/class/google_cloudbuild_trigger"/>
    <rdfs:range rdf:resource="http://www.w3.org/2001/XMLSchema#string"/>
  </owl:DatatypeProperty>
  <owl:DatatypeProperty rdf:about="http://example.org/onto/prop/google_cloudbuild_trigger_project_id">
    <rdfs:label>project_id</rdfs:label>
    <rdfs:comment>ID of the project that owns the Cloud Source Repository. If
omitted, the project ID requesting the build is assumed.</rdfs:comment>
    <rdfs:domain rdf:resource="http://example.org/onto/class/google_cloudbuild_trigger"/>
    <rdfs:range rdf:resource="http://www.w3.org/2001/XMLSchema#string"/>
  </owl:DatatypeProperty>
  <owl:DatatypeProperty rdf:about="http://example.org/onto/prop/google_cloudbuild_trigger_repo_name">
    <rdfs:label>repo_name</rdfs:label>
    <rdfs:comment>Name of the Cloud Source Repository. If omitted, the name "default" is assumed.</rdfs:comment>
    <rdfs:domain rdf:resource="http://example.org/onto/class/google_cloudbuild_trigger"/>
    <rdfs:range rdf:resource="http://www.w3.org/2001/XMLSchema#string"/>
  </owl:DatatypeProperty>
  <owl:DatatypeProperty rdf:about="http://example.org/onto/prop/google_cloudbuild_trigger_tag_name">
    <rdfs:label>tag_name</rdfs:label>
    <rdfs:comment>Name of the tag to build. Exactly one of a branch name, tag, or commit SHA must be provided.
This field is a regular expression.</rdfs:comment>
    <rdfs:domain rdf:resource="http://example.org/onto/class/google_cloudbuild_trigger"/>
    <rdfs:range rdf:resource="http://www.w3.org/2001/XMLSchema#string"/>
  </owl:DatatypeProperty>
  <owl:DatatypeProperty rdf:about="http://example.org/onto/prop/google_cloudbuild_trigger_secret">
    <rdfs:label>secret</rdfs:label>
    <rdfs:comment>Resource name for the secret required as a URL parameter.</rdfs:comment>
    <rdfs:domain rdf:resource="http://example.org/onto/class/google_cloudbuild_trigger"/>
    <rdfs:range rdf:resource="http://www.w3.org/2001/XMLSchema#string"/>
  </owl:DatatypeProperty>
  <owl:DatatypeProperty rdf:about="http://example.org/onto/prop/google_cloudbuild_trigger_state">
    <rdfs:label>state</rdfs:label>
    <rdfs:comment>Potential issues with the underlying Pub/Sub subscription configuration.
Only populated on get requests.</rdfs:comment>
    <rdfs:domain rdf:resource="http://example.org/onto/class/google_cloudbuild_trigger"/>
    <rdfs:range rdf:resource="http://www.w3.org/2001/XMLSchema#string"/>
  </owl:DatatypeProperty>
</rdf:RDF>
