<?xml version="1.0" encoding="UTF-8"?>
<rdf:RDF
  xmlns:rdf="http://www.w3.org/1999/02/22-rdf-syntax-ns#"
  xmlns:rdfs="http://www.w3.org/2000/01/rdf-schema#"
  xmlns:owl="http://www.w3.org/2002/07/owl#"
  xmlns:xsd="http://www.w3.org/2001/XMLSchema#"
  xml:base="http://example.org/onto/">
  <owl:Class rdf:about="http://example.org/onto/class/google_organization_access_approval_settings">
    <rdfs:label>google_organization_access_approval_settings</rdfs:label>
    <rdfs:comment>#
#     ***     AUTO GENERATED CODE    ***    Type: MMv1     ***
#
# ----------------------------------------------------------------------------
#
#     This code is generated by Magic Modules using the following:
#
#     Configuration: https:#github.com/GoogleCloudPlatform/magic-modules/tree/main/mmv1/products/accessapproval/OrganizationSettings.yaml
#     Template:      https:#github.com/GoogleCloudPlatform/magic-modules/tree/main/mmv1/templates/terraform/resource.html.markdown.tmpl
#
#     DO NOT EDIT this file directly. Any changes made to this file will be
#     overwritten during the next generation cycle.
#
# ----------------------------------------------------------------------------
subcategory: "Access Approval"
description: |-
  Access Approval enables you to require your explicit approval whenever Google support and engineering need to access your customer content.
---</rdfs:comment>
  </owl:Class>
  <owl:DatatypeProperty rdf:about="http://example.org/onto/prop/google_organization_access_approval_settings_active_key_version">
    <rdfs:label>active_key_version</rdfs:label>
    <rdfs:comment>The asymmetric crypto key version to use for signing approval requests.
Empty active_key_version indicates that a Google-managed key should be used for signing.</rdfs:comment>
    <rdfs:domain rdf:resource="http://example.org/onto/class/google_organization_access_approval_settings"/>
    <rdfs:range rdf:resource="http://www.w3.org/2001/XMLSchema#string"/>
  </owl:DatatypeProperty>
  <owl:DatatypeProperty rdf:about="http://example.org/onto/prop/google_organization_access_approval_settings_ancestor_has_active_key_version">
    <rdfs:label>ancestor_has_active_key_version</rdfs:label>
    <rdfs:comment>This field will always be unset for the organization since organizations do not have ancestors.</rdfs:comment>
    <rdfs:domain rdf:resource="http://example.org/onto/class/google_organization_access_approval_settings"/>
    <rdfs:range rdf:resource="http://www.w3.org/2001/XMLSchema#string"/>
  </owl:DatatypeProperty>
  <owl:DatatypeProperty rdf:about="http://example.org/onto/prop/google_organization_access_approval_settings_enrolled_ancestor">
    <rdfs:label>enrolled_ancestor</rdfs:label>
    <rdfs:comment>This field will always be unset for the organization since organizations do not have ancestors.</rdfs:comment>
    <rdfs:domain rdf:resource="http://example.org/onto/class/google_organization_access_approval_settings"/>
    <rdfs:range rdf:resource="http://www.w3.org/2001/XMLSchema#string"/>
  </owl:DatatypeProperty>
  <owl:DatatypeProperty rdf:about="http://example.org/onto/prop/google_organization_access_approval_settings_id">
    <rdfs:label>id</rdfs:label>
    <rdfs:domain rdf:resource="http://example.org/onto/class/google_organization_access_approval_settings"/>
    <rdfs:range rdf:resource="http://www.w3.org/2001/XMLSchema#string"/>
  </owl:DatatypeProperty>
  <owl:DatatypeProperty rdf:about="http://example.org/onto/prop/google_organization_access_approval_settings_invalid_key_version">
    <rdfs:label>invalid_key_version</rdfs:label>
    <rdfs:comment>If the field is true, that indicates that there is some configuration issue with the active_key_version
configured on this Organization (e.g. it doesn't exist or the Access Approval service account doesn't have the
correct permissions on it, etc.).</rdfs:comment>
    <rdfs:domain rdf:resource="http://example.org/onto/class/google_organization_access_approval_settings"/>
    <rdfs:range rdf:resource="http://www.w3.org/2001/XMLSchema#string"/>
  </owl:DatatypeProperty>
  <owl:DatatypeProperty rdf:about="http://example.org/onto/prop/google_organization_access_approval_settings_name">
    <rdfs:label>name</rdfs:label>
    <rdfs:comment>The resource name of the settings. Format is "organizations/{organization_id}/accessApprovalSettings"</rdfs:comment>
    <rdfs:domain rdf:resource="http://example.org/onto/class/google_organization_access_approval_settings"/>
    <rdfs:range rdf:resource="http://www.w3.org/2001/XMLSchema#string"/>
  </owl:DatatypeProperty>
  <owl:DatatypeProperty rdf:about="http://example.org/onto/prop/google_organization_access_approval_settings_notification_emails">
    <rdfs:label>notification_emails</rdfs:label>
    <rdfs:comment>A list of email addresses to which notifications relating to approval requests should be sent.
Notifications relating to a resource will be sent to all emails in the settings of ancestor
resources of that resource. A maximum of 50 email addresses are allowed.</rdfs:comment>
    <rdfs:domain rdf:resource="http://example.org/onto/class/google_organization_access_approval_settings"/>
    <rdfs:range rdf:resource="http://www.w3.org/2001/XMLSchema#string"/>
  </owl:DatatypeProperty>
  <owl:DatatypeProperty rdf:about="http://example.org/onto/prop/google_organization_access_approval_settings_organization_id">
    <rdfs:label>organization_id</rdfs:label>
    <rdfs:comment>ID of the organization of the access approval settings.</rdfs:comment>
    <rdfs:domain rdf:resource="http://example.org/onto/class/google_organization_access_approval_settings"/>
    <rdfs:range rdf:resource="http://www.w3.org/2001/XMLSchema#string"/>
  </owl:DatatypeProperty>
  <owl:DatatypeProperty rdf:about="http://example.org/onto/prop/google_organization_access_approval_settings_cloud_product">
    <rdfs:label>cloud_product</rdfs:label>
    <rdfs:comment>The product for which Access Approval will be enrolled. Allowed values are listed (case-sensitive):
  all
  appengine.googleapis.com
  bigquery.googleapis.com
  bigtable.googleapis.com
  cloudkms.googleapis.com
  compute.googleapis.com
  dataflow.googleapis.com
  iam.googleapis.com
  pubsub.googleapis.com
  storage.googleapis.com</rdfs:comment>
    <rdfs:domain rdf:resource="http://example.org/onto/class/google_organization_access_approval_settings"/>
    <rdfs:range rdf:resource="http://www.w3.org/2001/XMLSchema#string"/>
  </owl:DatatypeProperty>
  <owl:DatatypeProperty rdf:about="http://example.org/onto/prop/google_organization_access_approval_settings_enrollment_level">
    <rdfs:label>enrollment_level</rdfs:label>
    <rdfs:comment>The enrollment level of the service. Default value: "BLOCK_ALL" Possible values: ["BLOCK_ALL"]</rdfs:comment>
    <rdfs:domain rdf:resource="http://example.org/onto/class/google_organization_access_approval_settings"/>
    <rdfs:range rdf:resource="http://www.w3.org/2001/XMLSchema#string"/>
  </owl:DatatypeProperty>
  <owl:DatatypeProperty rdf:about="http://example.org/onto/prop/google_organization_access_approval_settings_create">
    <rdfs:label>create</rdfs:label>
    <rdfs:domain rdf:resource="http://example.org/onto/class/google_organization_access_approval_settings"/>
    <rdfs:range rdf:resource="http://www.w3.org/2001/XMLSchema#string"/>
  </owl:DatatypeProperty>
  <owl:DatatypeProperty rdf:about="http://example.org/onto/prop/google_organization_access_approval_settings_delete">
    <rdfs:label>delete</rdfs:label>
    <rdfs:domain rdf:resource="http://example.org/onto/class/google_organization_access_approval_settings"/>
    <rdfs:range rdf:resource="http://www.w3.org/2001/XMLSchema#string"/>
  </owl:DatatypeProperty>
  <owl:DatatypeProperty rdf:about="http://example.org/onto/prop/google_organization_access_approval_settings_update">
    <rdfs:label>update</rdfs:label>
    <rdfs:domain rdf:resource="http://example.org/onto/class/google_organization_access_approval_settings"/>
    <rdfs:range rdf:resource="http://www.w3.org/2001/XMLSchema#string"/>
  </owl:DatatypeProperty>
</rdf:RDF>
