<?xml version="1.0" encoding="UTF-8"?>
<rdf:RDF
  xmlns:rdf="http://www.w3.org/1999/02/22-rdf-syntax-ns#"
  xmlns:rdfs="http://www.w3.org/2000/01/rdf-schema#"
  xmlns:owl="http://www.w3.org/2002/07/owl#"
  xmlns:xsd="http://www.w3.org/2001/XMLSchema#"
  xml:base="http://example.org/onto/">
  <owl:Class rdf:about="http://example.org/onto/class/google_document_ai_warehouse_location">
    <rdfs:label>google_document_ai_warehouse_location</rdfs:label>
    <rdfs:comment>#
#     ***     AUTO GENERATED CODE    ***    Type: MMv1     ***
#
# ----------------------------------------------------------------------------
#
#     This code is generated by Magic Modules using the following:
#
#     Configuration: https:#github.com/GoogleCloudPlatform/magic-modules/tree/main/mmv1/products/documentaiwarehouse/Location.yaml
#     Template:      https:#github.com/GoogleCloudPlatform/magic-modules/tree/main/mmv1/templates/terraform/resource.html.markdown.tmpl
#
#     DO NOT EDIT this file directly. Any changes made to this file will be
#     overwritten during the next generation cycle.
#
# ----------------------------------------------------------------------------
subcategory: "Document AI Warehouse"
description: |-
  A location is used to initialize a project.
---</rdfs:comment>
  </owl:Class>
  <owl:DatatypeProperty rdf:about="http://example.org/onto/prop/google_document_ai_warehouse_location_access_control_mode">
    <rdfs:label>access_control_mode</rdfs:label>
    <rdfs:comment>The access control mode for accessing the customer data. Possible values: ["ACL_MODE_DOCUMENT_LEVEL_ACCESS_CONTROL_GCI", "ACL_MODE_DOCUMENT_LEVEL_ACCESS_CONTROL_BYOID", "ACL_MODE_UNIVERSAL_ACCESS"]</rdfs:comment>
    <rdfs:domain rdf:resource="http://example.org/onto/class/google_document_ai_warehouse_location"/>
    <rdfs:range rdf:resource="http://www.w3.org/2001/XMLSchema#string"/>
  </owl:DatatypeProperty>
  <owl:DatatypeProperty rdf:about="http://example.org/onto/prop/google_document_ai_warehouse_location_database_type">
    <rdfs:label>database_type</rdfs:label>
    <rdfs:comment>The type of database used to store customer data. Possible values: ["DB_INFRA_SPANNER", "DB_CLOUD_SQL_POSTGRES"]</rdfs:comment>
    <rdfs:domain rdf:resource="http://example.org/onto/class/google_document_ai_warehouse_location"/>
    <rdfs:range rdf:resource="http://www.w3.org/2001/XMLSchema#string"/>
  </owl:DatatypeProperty>
  <owl:DatatypeProperty rdf:about="http://example.org/onto/prop/google_document_ai_warehouse_location_document_creator_default_role">
    <rdfs:label>document_creator_default_role</rdfs:label>
    <rdfs:comment>The default role for the person who create a document. Possible values: ["DOCUMENT_ADMIN", "DOCUMENT_EDITOR", "DOCUMENT_VIEWER"]</rdfs:comment>
    <rdfs:domain rdf:resource="http://example.org/onto/class/google_document_ai_warehouse_location"/>
    <rdfs:range rdf:resource="http://www.w3.org/2001/XMLSchema#string"/>
  </owl:DatatypeProperty>
  <owl:DatatypeProperty rdf:about="http://example.org/onto/prop/google_document_ai_warehouse_location_id">
    <rdfs:label>id</rdfs:label>
    <rdfs:domain rdf:resource="http://example.org/onto/class/google_document_ai_warehouse_location"/>
    <rdfs:range rdf:resource="http://www.w3.org/2001/XMLSchema#string"/>
  </owl:DatatypeProperty>
  <owl:DatatypeProperty rdf:about="http://example.org/onto/prop/google_document_ai_warehouse_location_kms_key">
    <rdfs:label>kms_key</rdfs:label>
    <rdfs:comment>The KMS key used for CMEK encryption. It is required that
the kms key is in the same region as the endpoint. The
same key will be used for all provisioned resources, if
encryption is available. If the kmsKey is left empty, no
encryption will be enforced.</rdfs:comment>
    <rdfs:domain rdf:resource="http://example.org/onto/class/google_document_ai_warehouse_location"/>
    <rdfs:range rdf:resource="http://www.w3.org/2001/XMLSchema#string"/>
  </owl:DatatypeProperty>
  <owl:DatatypeProperty rdf:about="http://example.org/onto/prop/google_document_ai_warehouse_location_location">
    <rdfs:label>location</rdfs:label>
    <rdfs:comment>The location in which the instance is to be provisioned. It takes the form projects/{projectNumber}/locations/{location}.</rdfs:comment>
    <rdfs:domain rdf:resource="http://example.org/onto/class/google_document_ai_warehouse_location"/>
    <rdfs:range rdf:resource="http://www.w3.org/2001/XMLSchema#string"/>
  </owl:DatatypeProperty>
  <owl:DatatypeProperty rdf:about="http://example.org/onto/prop/google_document_ai_warehouse_location_project_number">
    <rdfs:label>project_number</rdfs:label>
    <rdfs:comment>The unique identifier of the project.</rdfs:comment>
    <rdfs:domain rdf:resource="http://example.org/onto/class/google_document_ai_warehouse_location"/>
    <rdfs:range rdf:resource="http://www.w3.org/2001/XMLSchema#string"/>
  </owl:DatatypeProperty>
  <owl:DatatypeProperty rdf:about="http://example.org/onto/prop/google_document_ai_warehouse_location_create">
    <rdfs:label>create</rdfs:label>
    <rdfs:domain rdf:resource="http://example.org/onto/class/google_document_ai_warehouse_location"/>
    <rdfs:range rdf:resource="http://www.w3.org/2001/XMLSchema#string"/>
  </owl:DatatypeProperty>
  <owl:DatatypeProperty rdf:about="http://example.org/onto/prop/google_document_ai_warehouse_location_delete">
    <rdfs:label>delete</rdfs:label>
    <rdfs:domain rdf:resource="http://example.org/onto/class/google_document_ai_warehouse_location"/>
    <rdfs:range rdf:resource="http://www.w3.org/2001/XMLSchema#string"/>
  </owl:DatatypeProperty>
</rdf:RDF>
