<?xml version="1.0" encoding="UTF-8"?>
<rdf:RDF
  xmlns:rdf="http://www.w3.org/1999/02/22-rdf-syntax-ns#"
  xmlns:rdfs="http://www.w3.org/2000/01/rdf-schema#"
  xmlns:owl="http://www.w3.org/2002/07/owl#"
  xmlns:xsd="http://www.w3.org/2001/XMLSchema#"
  xml:base="http://example.org/onto/">
  <owl:Class rdf:about="http://example.org/onto/class/google_firebase_data_connect_service">
    <rdfs:label>google_firebase_data_connect_service</rdfs:label>
    <rdfs:comment>#
#     ***     AUTO GENERATED CODE    ***    Type: MMv1     ***
#
# ----------------------------------------------------------------------------
#
#     This code is generated by Magic Modules using the following:
#
#     Configuration: https:#github.com/GoogleCloudPlatform/magic-modules/tree/main/mmv1/products/firebasedataconnect/Service.yaml
#     Template:      https:#github.com/GoogleCloudPlatform/magic-modules/tree/main/mmv1/templates/terraform/resource.html.markdown.tmpl
#
#     DO NOT EDIT this file directly. Any changes made to this file will be
#     overwritten during the next generation cycle.
#
# ----------------------------------------------------------------------------
subcategory: "Firebase Data Connect"
description: |-
  A Firebase Data Connect service.
---</rdfs:comment>
  </owl:Class>
  <owl:DatatypeProperty rdf:about="http://example.org/onto/prop/google_firebase_data_connect_service_annotations">
    <rdfs:label>annotations</rdfs:label>
    <rdfs:comment>Optional. Stores small amounts of arbitrary data.

**Note**: This field is non-authoritative, and will only manage the annotations present in your configuration.
Please refer to the field 'effective_annotations' for all of the annotations present on the resource.</rdfs:comment>
    <rdfs:domain rdf:resource="http://example.org/onto/class/google_firebase_data_connect_service"/>
    <rdfs:range rdf:resource="http://www.w3.org/2001/XMLSchema#string"/>
  </owl:DatatypeProperty>
  <owl:DatatypeProperty rdf:about="http://example.org/onto/prop/google_firebase_data_connect_service_create_time">
    <rdfs:label>create_time</rdfs:label>
    <rdfs:comment>Output only. [Output only] Create time stamp.</rdfs:comment>
    <rdfs:domain rdf:resource="http://example.org/onto/class/google_firebase_data_connect_service"/>
    <rdfs:range rdf:resource="http://www.w3.org/2001/XMLSchema#string"/>
  </owl:DatatypeProperty>
  <owl:DatatypeProperty rdf:about="http://example.org/onto/prop/google_firebase_data_connect_service_deletion_policy">
    <rdfs:label>deletion_policy</rdfs:label>
    <rdfs:comment>The deletion policy for the database. Setting the field to FORCE allows the
Service to be deleted even if a Schema or Connector is present. By default,
the Service deletion will only succeed when no Schema or Connectors are
present.
Possible values: DEFAULT, FORCE</rdfs:comment>
    <rdfs:domain rdf:resource="http://example.org/onto/class/google_firebase_data_connect_service"/>
    <rdfs:range rdf:resource="http://www.w3.org/2001/XMLSchema#string"/>
  </owl:DatatypeProperty>
  <owl:DatatypeProperty rdf:about="http://example.org/onto/prop/google_firebase_data_connect_service_display_name">
    <rdfs:label>display_name</rdfs:label>
    <rdfs:comment>Optional. Mutable human-readable name. 63 character limit.</rdfs:comment>
    <rdfs:domain rdf:resource="http://example.org/onto/class/google_firebase_data_connect_service"/>
    <rdfs:range rdf:resource="http://www.w3.org/2001/XMLSchema#string"/>
  </owl:DatatypeProperty>
  <owl:DatatypeProperty rdf:about="http://example.org/onto/prop/google_firebase_data_connect_service_effective_annotations">
    <rdfs:label>effective_annotations</rdfs:label>
    <rdfs:comment>All of annotations (key/value pairs) present on the resource in GCP, including the annotations configured through Terraform, other clients and services.</rdfs:comment>
    <rdfs:domain rdf:resource="http://example.org/onto/class/google_firebase_data_connect_service"/>
    <rdfs:range rdf:resource="http://www.w3.org/2001/XMLSchema#string"/>
  </owl:DatatypeProperty>
  <owl:DatatypeProperty rdf:about="http://example.org/onto/prop/google_firebase_data_connect_service_effective_labels">
    <rdfs:label>effective_labels</rdfs:label>
    <rdfs:comment>All of labels (key/value pairs) present on the resource in GCP, including the labels configured through Terraform, other clients and services.</rdfs:comment>
    <rdfs:domain rdf:resource="http://example.org/onto/class/google_firebase_data_connect_service"/>
    <rdfs:range rdf:resource="http://www.w3.org/2001/XMLSchema#string"/>
  </owl:DatatypeProperty>
  <owl:DatatypeProperty rdf:about="http://example.org/onto/prop/google_firebase_data_connect_service_etag">
    <rdfs:label>etag</rdfs:label>
    <rdfs:comment>Output only. This checksum is computed by the server based on the value of other
fields, and may be sent on update and delete requests to ensure the
client has an up-to-date value before proceeding.
[AIP-154](https://google.aip.dev/154)</rdfs:comment>
    <rdfs:domain rdf:resource="http://example.org/onto/class/google_firebase_data_connect_service"/>
    <rdfs:range rdf:resource="http://www.w3.org/2001/XMLSchema#string"/>
  </owl:DatatypeProperty>
  <owl:DatatypeProperty rdf:about="http://example.org/onto/prop/google_firebase_data_connect_service_id">
    <rdfs:label>id</rdfs:label>
    <rdfs:domain rdf:resource="http://example.org/onto/class/google_firebase_data_connect_service"/>
    <rdfs:range rdf:resource="http://www.w3.org/2001/XMLSchema#string"/>
  </owl:DatatypeProperty>
  <owl:DatatypeProperty rdf:about="http://example.org/onto/prop/google_firebase_data_connect_service_labels">
    <rdfs:label>labels</rdfs:label>
    <rdfs:comment>Optional. Labels as key value pairs.

**Note**: This field is non-authoritative, and will only manage the labels present in your configuration.
Please refer to the field 'effective_labels' for all of the labels present on the resource.</rdfs:comment>
    <rdfs:domain rdf:resource="http://example.org/onto/class/google_firebase_data_connect_service"/>
    <rdfs:range rdf:resource="http://www.w3.org/2001/XMLSchema#string"/>
  </owl:DatatypeProperty>
  <owl:DatatypeProperty rdf:about="http://example.org/onto/prop/google_firebase_data_connect_service_location">
    <rdfs:label>location</rdfs:label>
    <rdfs:comment>The region in which the service resides, e.g. "us-central1" or "asia-east1".</rdfs:comment>
    <rdfs:domain rdf:resource="http://example.org/onto/class/google_firebase_data_connect_service"/>
    <rdfs:range rdf:resource="http://www.w3.org/2001/XMLSchema#string"/>
  </owl:DatatypeProperty>
  <owl:DatatypeProperty rdf:about="http://example.org/onto/prop/google_firebase_data_connect_service_name">
    <rdfs:label>name</rdfs:label>
    <rdfs:comment>Identifier. The relative resource name of the Firebase Data Connect service, in the
format:
'''
projects/{project}/locations/{location}/services/{service}
'''
Note that the service ID is specific to Firebase Data Connect and does not
correspond to any of the instance IDs of the underlying data source
connections.</rdfs:comment>
    <rdfs:domain rdf:resource="http://example.org/onto/class/google_firebase_data_connect_service"/>
    <rdfs:range rdf:resource="http://www.w3.org/2001/XMLSchema#string"/>
  </owl:DatatypeProperty>
  <owl:DatatypeProperty rdf:about="http://example.org/onto/prop/google_firebase_data_connect_service_project">
    <rdfs:label>project</rdfs:label>
    <rdfs:domain rdf:resource="http://example.org/onto/class/google_firebase_data_connect_service"/>
    <rdfs:range rdf:resource="http://www.w3.org/2001/XMLSchema#string"/>
  </owl:DatatypeProperty>
  <owl:DatatypeProperty rdf:about="http://example.org/onto/prop/google_firebase_data_connect_service_reconciling">
    <rdfs:label>reconciling</rdfs:label>
    <rdfs:comment>Output only. A field that if true, indicates that the system is working update the
service.</rdfs:comment>
    <rdfs:domain rdf:resource="http://example.org/onto/class/google_firebase_data_connect_service"/>
    <rdfs:range rdf:resource="http://www.w3.org/2001/XMLSchema#string"/>
  </owl:DatatypeProperty>
  <owl:DatatypeProperty rdf:about="http://example.org/onto/prop/google_firebase_data_connect_service_service_id">
    <rdfs:label>service_id</rdfs:label>
    <rdfs:comment>Required. The ID to use for the service, which will become the final component of the
service's resource name.</rdfs:comment>
    <rdfs:domain rdf:resource="http://example.org/onto/class/google_firebase_data_connect_service"/>
    <rdfs:range rdf:resource="http://www.w3.org/2001/XMLSchema#string"/>
  </owl:DatatypeProperty>
  <owl:DatatypeProperty rdf:about="http://example.org/onto/prop/google_firebase_data_connect_service_terraform_labels">
    <rdfs:label>terraform_labels</rdfs:label>
    <rdfs:comment>The combination of labels configured directly on the resource
 and default labels configured on the provider.</rdfs:comment>
    <rdfs:domain rdf:resource="http://example.org/onto/class/google_firebase_data_connect_service"/>
    <rdfs:range rdf:resource="http://www.w3.org/2001/XMLSchema#string"/>
  </owl:DatatypeProperty>
  <owl:DatatypeProperty rdf:about="http://example.org/onto/prop/google_firebase_data_connect_service_uid">
    <rdfs:label>uid</rdfs:label>
    <rdfs:comment>Output only. System-assigned, unique identifier.</rdfs:comment>
    <rdfs:domain rdf:resource="http://example.org/onto/class/google_firebase_data_connect_service"/>
    <rdfs:range rdf:resource="http://www.w3.org/2001/XMLSchema#string"/>
  </owl:DatatypeProperty>
  <owl:DatatypeProperty rdf:about="http://example.org/onto/prop/google_firebase_data_connect_service_update_time">
    <rdfs:label>update_time</rdfs:label>
    <rdfs:comment>Output only. [Output only] Update time stamp.</rdfs:comment>
    <rdfs:domain rdf:resource="http://example.org/onto/class/google_firebase_data_connect_service"/>
    <rdfs:range rdf:resource="http://www.w3.org/2001/XMLSchema#string"/>
  </owl:DatatypeProperty>
  <owl:DatatypeProperty rdf:about="http://example.org/onto/prop/google_firebase_data_connect_service_create">
    <rdfs:label>create</rdfs:label>
    <rdfs:domain rdf:resource="http://example.org/onto/class/google_firebase_data_connect_service"/>
    <rdfs:range rdf:resource="http://www.w3.org/2001/XMLSchema#string"/>
  </owl:DatatypeProperty>
  <owl:DatatypeProperty rdf:about="http://example.org/onto/prop/google_firebase_data_connect_service_delete">
    <rdfs:label>delete</rdfs:label>
    <rdfs:domain rdf:resource="http://example.org/onto/class/google_firebase_data_connect_service"/>
    <rdfs:range rdf:resource="http://www.w3.org/2001/XMLSchema#string"/>
  </owl:DatatypeProperty>
  <owl:DatatypeProperty rdf:about="http://example.org/onto/prop/google_firebase_data_connect_service_update">
    <rdfs:label>update</rdfs:label>
    <rdfs:domain rdf:resource="http://example.org/onto/class/google_firebase_data_connect_service"/>
    <rdfs:range rdf:resource="http://www.w3.org/2001/XMLSchema#string"/>
  </owl:DatatypeProperty>
</rdf:RDF>
