<?xml version="1.0" encoding="UTF-8"?>
<rdf:RDF
  xmlns:rdf="http://www.w3.org/1999/02/22-rdf-syntax-ns#"
  xmlns:rdfs="http://www.w3.org/2000/01/rdf-schema#"
  xmlns:owl="http://www.w3.org/2002/07/owl#"
  xmlns:xsd="http://www.w3.org/2001/XMLSchema#"
  xml:base="http://example.org/onto/">
  <owl:Class rdf:about="http://example.org/onto/class/google_app_engine_flexible_app_version">
    <rdfs:label>google_app_engine_flexible_app_version</rdfs:label>
    <rdfs:comment>#
#     ***     AUTO GENERATED CODE    ***    Type: MMv1     ***
#
# ----------------------------------------------------------------------------
#
#     This code is generated by Magic Modules using the following:
#
#     Configuration: https:#github.com/GoogleCloudPlatform/magic-modules/tree/main/mmv1/products/appengine/FlexibleAppVersion.yaml
#     Template:      https:#github.com/GoogleCloudPlatform/magic-modules/tree/main/mmv1/templates/terraform/resource.html.markdown.tmpl
#
#     DO NOT EDIT this file directly. Any changes made to this file will be
#     overwritten during the next generation cycle.
#
# ----------------------------------------------------------------------------
subcategory: "App Engine"
description: |-
  Flexible App Version resource to create a new version of flexible GAE Application.
---</rdfs:comment>
  </owl:Class>
  <owl:DatatypeProperty rdf:about="http://example.org/onto/prop/google_app_engine_flexible_app_version_beta_settings">
    <rdfs:label>beta_settings</rdfs:label>
    <rdfs:comment>Metadata settings that are supplied to this version to enable beta runtime features.</rdfs:comment>
    <rdfs:domain rdf:resource="http://example.org/onto/class/google_app_engine_flexible_app_version"/>
    <rdfs:range rdf:resource="http://www.w3.org/2001/XMLSchema#string"/>
  </owl:DatatypeProperty>
  <owl:DatatypeProperty rdf:about="http://example.org/onto/prop/google_app_engine_flexible_app_version_default_expiration">
    <rdfs:label>default_expiration</rdfs:label>
    <rdfs:comment>Duration that static files should be cached by web proxies and browsers.
Only applicable if the corresponding StaticFilesHandler does not specify its own expiration time.</rdfs:comment>
    <rdfs:domain rdf:resource="http://example.org/onto/class/google_app_engine_flexible_app_version"/>
    <rdfs:range rdf:resource="http://www.w3.org/2001/XMLSchema#string"/>
  </owl:DatatypeProperty>
  <owl:DatatypeProperty rdf:about="http://example.org/onto/prop/google_app_engine_flexible_app_version_delete_service_on_destroy">
    <rdfs:label>delete_service_on_destroy</rdfs:label>
    <rdfs:comment>If set to 'true', the service will be deleted if it is the last version.</rdfs:comment>
    <rdfs:domain rdf:resource="http://example.org/onto/class/google_app_engine_flexible_app_version"/>
    <rdfs:range rdf:resource="http://www.w3.org/2001/XMLSchema#string"/>
  </owl:DatatypeProperty>
  <owl:DatatypeProperty rdf:about="http://example.org/onto/prop/google_app_engine_flexible_app_version_env_variables">
    <rdfs:label>env_variables</rdfs:label>
    <rdfs:comment>Environment variables available to the application.  As these are not returned in the API request, Terraform will not detect any changes made outside of the Terraform config.</rdfs:comment>
    <rdfs:domain rdf:resource="http://example.org/onto/class/google_app_engine_flexible_app_version"/>
    <rdfs:range rdf:resource="http://www.w3.org/2001/XMLSchema#string"/>
  </owl:DatatypeProperty>
  <owl:DatatypeProperty rdf:about="http://example.org/onto/prop/google_app_engine_flexible_app_version_id">
    <rdfs:label>id</rdfs:label>
    <rdfs:domain rdf:resource="http://example.org/onto/class/google_app_engine_flexible_app_version"/>
    <rdfs:range rdf:resource="http://www.w3.org/2001/XMLSchema#string"/>
  </owl:DatatypeProperty>
  <owl:DatatypeProperty rdf:about="http://example.org/onto/prop/google_app_engine_flexible_app_version_inbound_services">
    <rdfs:label>inbound_services</rdfs:label>
    <rdfs:comment>A list of the types of messages that this application is able to receive. Possible values: ["INBOUND_SERVICE_MAIL", "INBOUND_SERVICE_MAIL_BOUNCE", "INBOUND_SERVICE_XMPP_ERROR", "INBOUND_SERVICE_XMPP_MESSAGE", "INBOUND_SERVICE_XMPP_SUBSCRIBE", "INBOUND_SERVICE_XMPP_PRESENCE", "INBOUND_SERVICE_CHANNEL_PRESENCE", "INBOUND_SERVICE_WARMUP"]</rdfs:comment>
    <rdfs:domain rdf:resource="http://example.org/onto/class/google_app_engine_flexible_app_version"/>
    <rdfs:range rdf:resource="http://www.w3.org/2001/XMLSchema#string"/>
  </owl:DatatypeProperty>
  <owl:DatatypeProperty rdf:about="http://example.org/onto/prop/google_app_engine_flexible_app_version_instance_class">
    <rdfs:label>instance_class</rdfs:label>
    <rdfs:comment>Instance class that is used to run this version. Valid values are
AutomaticScaling: F1, F2, F4, F4_1G
ManualScaling: B1, B2, B4, B8, B4_1G
Defaults to F1 for AutomaticScaling and B1 for ManualScaling.</rdfs:comment>
    <rdfs:domain rdf:resource="http://example.org/onto/class/google_app_engine_flexible_app_version"/>
    <rdfs:range rdf:resource="http://www.w3.org/2001/XMLSchema#string"/>
  </owl:DatatypeProperty>
  <owl:DatatypeProperty rdf:about="http://example.org/onto/prop/google_app_engine_flexible_app_version_name">
    <rdfs:label>name</rdfs:label>
    <rdfs:comment>Full path to the Version resource in the API. Example, "v1".</rdfs:comment>
    <rdfs:domain rdf:resource="http://example.org/onto/class/google_app_engine_flexible_app_version"/>
    <rdfs:range rdf:resource="http://www.w3.org/2001/XMLSchema#string"/>
  </owl:DatatypeProperty>
  <owl:DatatypeProperty rdf:about="http://example.org/onto/prop/google_app_engine_flexible_app_version_nobuild_files_regex">
    <rdfs:label>nobuild_files_regex</rdfs:label>
    <rdfs:comment>Files that match this pattern will not be built into this version. Only applicable for Go runtimes.</rdfs:comment>
    <rdfs:domain rdf:resource="http://example.org/onto/class/google_app_engine_flexible_app_version"/>
    <rdfs:range rdf:resource="http://www.w3.org/2001/XMLSchema#string"/>
  </owl:DatatypeProperty>
  <owl:DatatypeProperty rdf:about="http://example.org/onto/prop/google_app_engine_flexible_app_version_noop_on_destroy">
    <rdfs:label>noop_on_destroy</rdfs:label>
    <rdfs:comment>If set to 'true', the application version will not be deleted.</rdfs:comment>
    <rdfs:domain rdf:resource="http://example.org/onto/class/google_app_engine_flexible_app_version"/>
    <rdfs:range rdf:resource="http://www.w3.org/2001/XMLSchema#string"/>
  </owl:DatatypeProperty>
  <owl:DatatypeProperty rdf:about="http://example.org/onto/prop/google_app_engine_flexible_app_version_project">
    <rdfs:label>project</rdfs:label>
    <rdfs:domain rdf:resource="http://example.org/onto/class/google_app_engine_flexible_app_version"/>
    <rdfs:range rdf:resource="http://www.w3.org/2001/XMLSchema#string"/>
  </owl:DatatypeProperty>
  <owl:DatatypeProperty rdf:about="http://example.org/onto/prop/google_app_engine_flexible_app_version_runtime">
    <rdfs:label>runtime</rdfs:label>
    <rdfs:comment>Desired runtime. Example python27.</rdfs:comment>
    <rdfs:domain rdf:resource="http://example.org/onto/class/google_app_engine_flexible_app_version"/>
    <rdfs:range rdf:resource="http://www.w3.org/2001/XMLSchema#string"/>
  </owl:DatatypeProperty>
  <owl:DatatypeProperty rdf:about="http://example.org/onto/prop/google_app_engine_flexible_app_version_runtime_api_version">
    <rdfs:label>runtime_api_version</rdfs:label>
    <rdfs:comment>The version of the API in the given runtime environment.
Please see the app.yaml reference for valid values at 'https://cloud.google.com/appengine/docs/standard/<language>/config/appref'\
Substitute '<language>' with 'python', 'java', 'php', 'ruby', 'go' or 'nodejs'.</rdfs:comment>
    <rdfs:domain rdf:resource="http://example.org/onto/class/google_app_engine_flexible_app_version"/>
    <rdfs:range rdf:resource="http://www.w3.org/2001/XMLSchema#string"/>
  </owl:DatatypeProperty>
  <owl:DatatypeProperty rdf:about="http://example.org/onto/prop/google_app_engine_flexible_app_version_runtime_channel">
    <rdfs:label>runtime_channel</rdfs:label>
    <rdfs:comment>The channel of the runtime to use. Only available for some runtimes.</rdfs:comment>
    <rdfs:domain rdf:resource="http://example.org/onto/class/google_app_engine_flexible_app_version"/>
    <rdfs:range rdf:resource="http://www.w3.org/2001/XMLSchema#string"/>
  </owl:DatatypeProperty>
  <owl:DatatypeProperty rdf:about="http://example.org/onto/prop/google_app_engine_flexible_app_version_runtime_main_executable_path">
    <rdfs:label>runtime_main_executable_path</rdfs:label>
    <rdfs:comment>The path or name of the app's main executable.</rdfs:comment>
    <rdfs:domain rdf:resource="http://example.org/onto/class/google_app_engine_flexible_app_version"/>
    <rdfs:range rdf:resource="http://www.w3.org/2001/XMLSchema#string"/>
  </owl:DatatypeProperty>
  <owl:DatatypeProperty rdf:about="http://example.org/onto/prop/google_app_engine_flexible_app_version_service">
    <rdfs:label>service</rdfs:label>
    <rdfs:comment>AppEngine service resource. Can contain numbers, letters, and hyphens.</rdfs:comment>
    <rdfs:domain rdf:resource="http://example.org/onto/class/google_app_engine_flexible_app_version"/>
    <rdfs:range rdf:resource="http://www.w3.org/2001/XMLSchema#string"/>
  </owl:DatatypeProperty>
  <owl:DatatypeProperty rdf:about="http://example.org/onto/prop/google_app_engine_flexible_app_version_service_account">
    <rdfs:label>service_account</rdfs:label>
    <rdfs:comment>The identity that the deployed version will run as. Admin API will use the App Engine Appspot service account as
default if this field is neither provided in app.yaml file nor through CLI flag.</rdfs:comment>
    <rdfs:domain rdf:resource="http://example.org/onto/class/google_app_engine_flexible_app_version"/>
    <rdfs:range rdf:resource="http://www.w3.org/2001/XMLSchema#string"/>
  </owl:DatatypeProperty>
  <owl:DatatypeProperty rdf:about="http://example.org/onto/prop/google_app_engine_flexible_app_version_serving_status">
    <rdfs:label>serving_status</rdfs:label>
    <rdfs:comment>Current serving status of this version. Only the versions with a SERVING status create instances and can be billed. Default value: "SERVING" Possible values: ["SERVING", "STOPPED"]</rdfs:comment>
    <rdfs:domain rdf:resource="http://example.org/onto/class/google_app_engine_flexible_app_version"/>
    <rdfs:range rdf:resource="http://www.w3.org/2001/XMLSchema#string"/>
  </owl:DatatypeProperty>
  <owl:DatatypeProperty rdf:about="http://example.org/onto/prop/google_app_engine_flexible_app_version_version_id">
    <rdfs:label>version_id</rdfs:label>
    <rdfs:comment>Relative name of the version within the service. For example, 'v1'. Version names can contain only lowercase letters, numbers, or hyphens.
Reserved names,"default", "latest", and any name with the prefix "ah-".</rdfs:comment>
    <rdfs:domain rdf:resource="http://example.org/onto/class/google_app_engine_flexible_app_version"/>
    <rdfs:range rdf:resource="http://www.w3.org/2001/XMLSchema#string"/>
  </owl:DatatypeProperty>
  <owl:DatatypeProperty rdf:about="http://example.org/onto/prop/google_app_engine_flexible_app_version_auth_fail_action">
    <rdfs:label>auth_fail_action</rdfs:label>
    <rdfs:comment>Action to take when users access resources that require authentication. Default value: "AUTH_FAIL_ACTION_REDIRECT" Possible values: ["AUTH_FAIL_ACTION_REDIRECT", "AUTH_FAIL_ACTION_UNAUTHORIZED"]</rdfs:comment>
    <rdfs:domain rdf:resource="http://example.org/onto/class/google_app_engine_flexible_app_version"/>
    <rdfs:range rdf:resource="http://www.w3.org/2001/XMLSchema#string"/>
  </owl:DatatypeProperty>
  <owl:DatatypeProperty rdf:about="http://example.org/onto/prop/google_app_engine_flexible_app_version_login">
    <rdfs:label>login</rdfs:label>
    <rdfs:comment>Level of login required to access this resource. Default value: "LOGIN_OPTIONAL" Possible values: ["LOGIN_OPTIONAL", "LOGIN_ADMIN", "LOGIN_REQUIRED"]</rdfs:comment>
    <rdfs:domain rdf:resource="http://example.org/onto/class/google_app_engine_flexible_app_version"/>
    <rdfs:range rdf:resource="http://www.w3.org/2001/XMLSchema#string"/>
  </owl:DatatypeProperty>
  <owl:DatatypeProperty rdf:about="http://example.org/onto/prop/google_app_engine_flexible_app_version_script">
    <rdfs:label>script</rdfs:label>
    <rdfs:comment>Path to the script from the application root directory.</rdfs:comment>
    <rdfs:domain rdf:resource="http://example.org/onto/class/google_app_engine_flexible_app_version"/>
    <rdfs:range rdf:resource="http://www.w3.org/2001/XMLSchema#string"/>
  </owl:DatatypeProperty>
  <owl:DatatypeProperty rdf:about="http://example.org/onto/prop/google_app_engine_flexible_app_version_security_level">
    <rdfs:label>security_level</rdfs:label>
    <rdfs:comment>Security (HTTPS) enforcement for this URL. Possible values: ["SECURE_DEFAULT", "SECURE_NEVER", "SECURE_OPTIONAL", "SECURE_ALWAYS"]</rdfs:comment>
    <rdfs:domain rdf:resource="http://example.org/onto/class/google_app_engine_flexible_app_version"/>
    <rdfs:range rdf:resource="http://www.w3.org/2001/XMLSchema#string"/>
  </owl:DatatypeProperty>
  <owl:DatatypeProperty rdf:about="http://example.org/onto/prop/google_app_engine_flexible_app_version_url">
    <rdfs:label>url</rdfs:label>
    <rdfs:comment>URL to serve the endpoint at.</rdfs:comment>
    <rdfs:domain rdf:resource="http://example.org/onto/class/google_app_engine_flexible_app_version"/>
    <rdfs:range rdf:resource="http://www.w3.org/2001/XMLSchema#string"/>
  </owl:DatatypeProperty>
  <owl:DatatypeProperty rdf:about="http://example.org/onto/prop/google_app_engine_flexible_app_version_cool_down_period">
    <rdfs:label>cool_down_period</rdfs:label>
    <rdfs:comment>The time period that the Autoscaler should wait before it starts collecting information from a new instance.
This prevents the autoscaler from collecting information when the instance is initializing,
during which the collected usage would not be reliable. Default: 120s</rdfs:comment>
    <rdfs:domain rdf:resource="http://example.org/onto/class/google_app_engine_flexible_app_version"/>
    <rdfs:range rdf:resource="http://www.w3.org/2001/XMLSchema#string"/>
  </owl:DatatypeProperty>
  <owl:DatatypeProperty rdf:about="http://example.org/onto/prop/google_app_engine_flexible_app_version_max_concurrent_requests">
    <rdfs:label>max_concurrent_requests</rdfs:label>
    <rdfs:comment>Number of concurrent requests an automatic scaling instance can accept before the scheduler spawns a new instance.

Defaults to a runtime-specific value.</rdfs:comment>
    <rdfs:domain rdf:resource="http://example.org/onto/class/google_app_engine_flexible_app_version"/>
    <rdfs:range rdf:resource="http://www.w3.org/2001/XMLSchema#string"/>
  </owl:DatatypeProperty>
  <owl:DatatypeProperty rdf:about="http://example.org/onto/prop/google_app_engine_flexible_app_version_max_idle_instances">
    <rdfs:label>max_idle_instances</rdfs:label>
    <rdfs:comment>Maximum number of idle instances that should be maintained for this version.</rdfs:comment>
    <rdfs:domain rdf:resource="http://example.org/onto/class/google_app_engine_flexible_app_version"/>
    <rdfs:range rdf:resource="http://www.w3.org/2001/XMLSchema#string"/>
  </owl:DatatypeProperty>
  <owl:DatatypeProperty rdf:about="http://example.org/onto/prop/google_app_engine_flexible_app_version_max_pending_latency">
    <rdfs:label>max_pending_latency</rdfs:label>
    <rdfs:comment>Maximum amount of time that a request should wait in the pending queue before starting a new instance to handle it.</rdfs:comment>
    <rdfs:domain rdf:resource="http://example.org/onto/class/google_app_engine_flexible_app_version"/>
    <rdfs:range rdf:resource="http://www.w3.org/2001/XMLSchema#string"/>
  </owl:DatatypeProperty>
  <owl:DatatypeProperty rdf:about="http://example.org/onto/prop/google_app_engine_flexible_app_version_max_total_instances">
    <rdfs:label>max_total_instances</rdfs:label>
    <rdfs:comment>Maximum number of instances that should be started to handle requests for this version. Default: 20</rdfs:comment>
    <rdfs:domain rdf:resource="http://example.org/onto/class/google_app_engine_flexible_app_version"/>
    <rdfs:range rdf:resource="http://www.w3.org/2001/XMLSchema#string"/>
  </owl:DatatypeProperty>
  <owl:DatatypeProperty rdf:about="http://example.org/onto/prop/google_app_engine_flexible_app_version_min_idle_instances">
    <rdfs:label>min_idle_instances</rdfs:label>
    <rdfs:comment>Minimum number of idle instances that should be maintained for this version. Only applicable for the default version of a service.</rdfs:comment>
    <rdfs:domain rdf:resource="http://example.org/onto/class/google_app_engine_flexible_app_version"/>
    <rdfs:range rdf:resource="http://www.w3.org/2001/XMLSchema#string"/>
  </owl:DatatypeProperty>
  <owl:DatatypeProperty rdf:about="http://example.org/onto/prop/google_app_engine_flexible_app_version_min_pending_latency">
    <rdfs:label>min_pending_latency</rdfs:label>
    <rdfs:comment>Minimum amount of time a request should wait in the pending queue before starting a new instance to handle it.</rdfs:comment>
    <rdfs:domain rdf:resource="http://example.org/onto/class/google_app_engine_flexible_app_version"/>
    <rdfs:range rdf:resource="http://www.w3.org/2001/XMLSchema#string"/>
  </owl:DatatypeProperty>
  <owl:DatatypeProperty rdf:about="http://example.org/onto/prop/google_app_engine_flexible_app_version_min_total_instances">
    <rdfs:label>min_total_instances</rdfs:label>
    <rdfs:comment>Minimum number of running instances that should be maintained for this version. Default: 2</rdfs:comment>
    <rdfs:domain rdf:resource="http://example.org/onto/class/google_app_engine_flexible_app_version"/>
    <rdfs:range rdf:resource="http://www.w3.org/2001/XMLSchema#string"/>
  </owl:DatatypeProperty>
  <owl:DatatypeProperty rdf:about="http://example.org/onto/prop/google_app_engine_flexible_app_version_aggregation_window_length">
    <rdfs:label>aggregation_window_length</rdfs:label>
    <rdfs:comment>Period of time over which CPU utilization is calculated.</rdfs:comment>
    <rdfs:domain rdf:resource="http://example.org/onto/class/google_app_engine_flexible_app_version"/>
    <rdfs:range rdf:resource="http://www.w3.org/2001/XMLSchema#string"/>
  </owl:DatatypeProperty>
  <owl:DatatypeProperty rdf:about="http://example.org/onto/prop/google_app_engine_flexible_app_version_target_utilization">
    <rdfs:label>target_utilization</rdfs:label>
    <rdfs:comment>Target CPU utilization ratio to maintain when scaling. Must be between 0 and 1.</rdfs:comment>
    <rdfs:domain rdf:resource="http://example.org/onto/class/google_app_engine_flexible_app_version"/>
    <rdfs:range rdf:resource="http://www.w3.org/2001/XMLSchema#string"/>
  </owl:DatatypeProperty>
  <owl:DatatypeProperty rdf:about="http://example.org/onto/prop/google_app_engine_flexible_app_version_target_read_bytes_per_second">
    <rdfs:label>target_read_bytes_per_second</rdfs:label>
    <rdfs:comment>Target bytes read per second.</rdfs:comment>
    <rdfs:domain rdf:resource="http://example.org/onto/class/google_app_engine_flexible_app_version"/>
    <rdfs:range rdf:resource="http://www.w3.org/2001/XMLSchema#string"/>
  </owl:DatatypeProperty>
  <owl:DatatypeProperty rdf:about="http://example.org/onto/prop/google_app_engine_flexible_app_version_target_read_ops_per_second">
    <rdfs:label>target_read_ops_per_second</rdfs:label>
    <rdfs:comment>Target ops read per seconds.</rdfs:comment>
    <rdfs:domain rdf:resource="http://example.org/onto/class/google_app_engine_flexible_app_version"/>
    <rdfs:range rdf:resource="http://www.w3.org/2001/XMLSchema#string"/>
  </owl:DatatypeProperty>
  <owl:DatatypeProperty rdf:about="http://example.org/onto/prop/google_app_engine_flexible_app_version_target_write_bytes_per_second">
    <rdfs:label>target_write_bytes_per_second</rdfs:label>
    <rdfs:comment>Target bytes written per second.</rdfs:comment>
    <rdfs:domain rdf:resource="http://example.org/onto/class/google_app_engine_flexible_app_version"/>
    <rdfs:range rdf:resource="http://www.w3.org/2001/XMLSchema#string"/>
  </owl:DatatypeProperty>
  <owl:DatatypeProperty rdf:about="http://example.org/onto/prop/google_app_engine_flexible_app_version_target_write_ops_per_second">
    <rdfs:label>target_write_ops_per_second</rdfs:label>
    <rdfs:comment>Target ops written per second.</rdfs:comment>
    <rdfs:domain rdf:resource="http://example.org/onto/class/google_app_engine_flexible_app_version"/>
    <rdfs:range rdf:resource="http://www.w3.org/2001/XMLSchema#string"/>
  </owl:DatatypeProperty>
  <owl:DatatypeProperty rdf:about="http://example.org/onto/prop/google_app_engine_flexible_app_version_target_received_bytes_per_second">
    <rdfs:label>target_received_bytes_per_second</rdfs:label>
    <rdfs:comment>Target bytes received per second.</rdfs:comment>
    <rdfs:domain rdf:resource="http://example.org/onto/class/google_app_engine_flexible_app_version"/>
    <rdfs:range rdf:resource="http://www.w3.org/2001/XMLSchema#string"/>
  </owl:DatatypeProperty>
  <owl:DatatypeProperty rdf:about="http://example.org/onto/prop/google_app_engine_flexible_app_version_target_received_packets_per_second">
    <rdfs:label>target_received_packets_per_second</rdfs:label>
    <rdfs:comment>Target packets received per second.</rdfs:comment>
    <rdfs:domain rdf:resource="http://example.org/onto/class/google_app_engine_flexible_app_version"/>
    <rdfs:range rdf:resource="http://www.w3.org/2001/XMLSchema#string"/>
  </owl:DatatypeProperty>
  <owl:DatatypeProperty rdf:about="http://example.org/onto/prop/google_app_engine_flexible_app_version_target_sent_bytes_per_second">
    <rdfs:label>target_sent_bytes_per_second</rdfs:label>
    <rdfs:comment>Target bytes sent per second.</rdfs:comment>
    <rdfs:domain rdf:resource="http://example.org/onto/class/google_app_engine_flexible_app_version"/>
    <rdfs:range rdf:resource="http://www.w3.org/2001/XMLSchema#string"/>
  </owl:DatatypeProperty>
  <owl:DatatypeProperty rdf:about="http://example.org/onto/prop/google_app_engine_flexible_app_version_target_sent_packets_per_second">
    <rdfs:label>target_sent_packets_per_second</rdfs:label>
    <rdfs:comment>Target packets sent per second.</rdfs:comment>
    <rdfs:domain rdf:resource="http://example.org/onto/class/google_app_engine_flexible_app_version"/>
    <rdfs:range rdf:resource="http://www.w3.org/2001/XMLSchema#string"/>
  </owl:DatatypeProperty>
  <owl:DatatypeProperty rdf:about="http://example.org/onto/prop/google_app_engine_flexible_app_version_target_concurrent_requests">
    <rdfs:label>target_concurrent_requests</rdfs:label>
    <rdfs:comment>Target number of concurrent requests.</rdfs:comment>
    <rdfs:domain rdf:resource="http://example.org/onto/class/google_app_engine_flexible_app_version"/>
    <rdfs:range rdf:resource="http://www.w3.org/2001/XMLSchema#string"/>
  </owl:DatatypeProperty>
  <owl:DatatypeProperty rdf:about="http://example.org/onto/prop/google_app_engine_flexible_app_version_target_request_count_per_second">
    <rdfs:label>target_request_count_per_second</rdfs:label>
    <rdfs:comment>Target requests per second.</rdfs:comment>
    <rdfs:domain rdf:resource="http://example.org/onto/class/google_app_engine_flexible_app_version"/>
    <rdfs:range rdf:resource="http://www.w3.org/2001/XMLSchema#string"/>
  </owl:DatatypeProperty>
  <owl:DatatypeProperty rdf:about="http://example.org/onto/prop/google_app_engine_flexible_app_version_app_yaml_path">
    <rdfs:label>app_yaml_path</rdfs:label>
    <rdfs:comment>Path to the yaml file used in deployment, used to determine runtime configuration details.</rdfs:comment>
    <rdfs:domain rdf:resource="http://example.org/onto/class/google_app_engine_flexible_app_version"/>
    <rdfs:range rdf:resource="http://www.w3.org/2001/XMLSchema#string"/>
  </owl:DatatypeProperty>
  <owl:DatatypeProperty rdf:about="http://example.org/onto/prop/google_app_engine_flexible_app_version_cloud_build_timeout">
    <rdfs:label>cloud_build_timeout</rdfs:label>
    <rdfs:comment>The Cloud Build timeout used as part of any dependent builds performed by version creation. Defaults to 10 minutes.

A duration in seconds with up to nine fractional digits, terminated by 's'. Example: "3.5s".</rdfs:comment>
    <rdfs:domain rdf:resource="http://example.org/onto/class/google_app_engine_flexible_app_version"/>
    <rdfs:range rdf:resource="http://www.w3.org/2001/XMLSchema#string"/>
  </owl:DatatypeProperty>
  <owl:DatatypeProperty rdf:about="http://example.org/onto/prop/google_app_engine_flexible_app_version_image">
    <rdfs:label>image</rdfs:label>
    <rdfs:comment>URI to the hosted container image in Google Container Registry. The URI must be fully qualified and include a tag or digest.
Examples: "gcr.io/my-project/image:tag" or "gcr.io/my-project/image@digest"</rdfs:comment>
    <rdfs:domain rdf:resource="http://example.org/onto/class/google_app_engine_flexible_app_version"/>
    <rdfs:range rdf:resource="http://www.w3.org/2001/XMLSchema#string"/>
  </owl:DatatypeProperty>
  <owl:DatatypeProperty rdf:about="http://example.org/onto/prop/google_app_engine_flexible_app_version_name">
    <rdfs:label>name</rdfs:label>
    <rdfs:domain rdf:resource="http://example.org/onto/class/google_app_engine_flexible_app_version"/>
    <rdfs:range rdf:resource="http://www.w3.org/2001/XMLSchema#string"/>
  </owl:DatatypeProperty>
  <owl:DatatypeProperty rdf:about="http://example.org/onto/prop/google_app_engine_flexible_app_version_sha1_sum">
    <rdfs:label>sha1_sum</rdfs:label>
    <rdfs:comment>SHA1 checksum of the file</rdfs:comment>
    <rdfs:domain rdf:resource="http://example.org/onto/class/google_app_engine_flexible_app_version"/>
    <rdfs:range rdf:resource="http://www.w3.org/2001/XMLSchema#string"/>
  </owl:DatatypeProperty>
  <owl:DatatypeProperty rdf:about="http://example.org/onto/prop/google_app_engine_flexible_app_version_source_url">
    <rdfs:label>source_url</rdfs:label>
    <rdfs:comment>Source URL</rdfs:comment>
    <rdfs:domain rdf:resource="http://example.org/onto/class/google_app_engine_flexible_app_version"/>
    <rdfs:range rdf:resource="http://www.w3.org/2001/XMLSchema#string"/>
  </owl:DatatypeProperty>
  <owl:DatatypeProperty rdf:about="http://example.org/onto/prop/google_app_engine_flexible_app_version_files_count">
    <rdfs:label>files_count</rdfs:label>
    <rdfs:comment>files count</rdfs:comment>
    <rdfs:domain rdf:resource="http://example.org/onto/class/google_app_engine_flexible_app_version"/>
    <rdfs:range rdf:resource="http://www.w3.org/2001/XMLSchema#string"/>
  </owl:DatatypeProperty>
  <owl:DatatypeProperty rdf:about="http://example.org/onto/prop/google_app_engine_flexible_app_version_source_url">
    <rdfs:label>source_url</rdfs:label>
    <rdfs:comment>Source URL</rdfs:comment>
    <rdfs:domain rdf:resource="http://example.org/onto/class/google_app_engine_flexible_app_version"/>
    <rdfs:range rdf:resource="http://www.w3.org/2001/XMLSchema#string"/>
  </owl:DatatypeProperty>
  <owl:DatatypeProperty rdf:about="http://example.org/onto/prop/google_app_engine_flexible_app_version_config_id">
    <rdfs:label>config_id</rdfs:label>
    <rdfs:comment>Endpoints service configuration ID as specified by the Service Management API. For example "2016-09-19r1".

By default, the rollout strategy for Endpoints is "FIXED". This means that Endpoints starts up with a particular configuration ID.
When a new configuration is rolled out, Endpoints must be given the new configuration ID. The configId field is used to give the configuration ID
and is required in this case.

Endpoints also has a rollout strategy called "MANAGED". When using this, Endpoints fetches the latest configuration and does not need
the configuration ID. In this case, configId must be omitted.</rdfs:comment>
    <rdfs:domain rdf:resource="http://example.org/onto/class/google_app_engine_flexible_app_version"/>
    <rdfs:range rdf:resource="http://www.w3.org/2001/XMLSchema#string"/>
  </owl:DatatypeProperty>
  <owl:DatatypeProperty rdf:about="http://example.org/onto/prop/google_app_engine_flexible_app_version_disable_trace_sampling">
    <rdfs:label>disable_trace_sampling</rdfs:label>
    <rdfs:comment>Enable or disable trace sampling. By default, this is set to false for enabled.</rdfs:comment>
    <rdfs:domain rdf:resource="http://example.org/onto/class/google_app_engine_flexible_app_version"/>
    <rdfs:range rdf:resource="http://www.w3.org/2001/XMLSchema#string"/>
  </owl:DatatypeProperty>
  <owl:DatatypeProperty rdf:about="http://example.org/onto/prop/google_app_engine_flexible_app_version_name">
    <rdfs:label>name</rdfs:label>
    <rdfs:comment>Endpoints service name which is the name of the "service" resource in the Service Management API.
For example "myapi.endpoints.myproject.cloud.goog"</rdfs:comment>
    <rdfs:domain rdf:resource="http://example.org/onto/class/google_app_engine_flexible_app_version"/>
    <rdfs:range rdf:resource="http://www.w3.org/2001/XMLSchema#string"/>
  </owl:DatatypeProperty>
  <owl:DatatypeProperty rdf:about="http://example.org/onto/prop/google_app_engine_flexible_app_version_rollout_strategy">
    <rdfs:label>rollout_strategy</rdfs:label>
    <rdfs:comment>Endpoints rollout strategy. If FIXED, configId must be specified. If MANAGED, configId must be omitted. Default value: "FIXED" Possible values: ["FIXED", "MANAGED"]</rdfs:comment>
    <rdfs:domain rdf:resource="http://example.org/onto/class/google_app_engine_flexible_app_version"/>
    <rdfs:range rdf:resource="http://www.w3.org/2001/XMLSchema#string"/>
  </owl:DatatypeProperty>
  <owl:DatatypeProperty rdf:about="http://example.org/onto/prop/google_app_engine_flexible_app_version_shell">
    <rdfs:label>shell</rdfs:label>
    <rdfs:comment>The format should be a shell command that can be fed to bash -c.</rdfs:comment>
    <rdfs:domain rdf:resource="http://example.org/onto/class/google_app_engine_flexible_app_version"/>
    <rdfs:range rdf:resource="http://www.w3.org/2001/XMLSchema#string"/>
  </owl:DatatypeProperty>
  <owl:DatatypeProperty rdf:about="http://example.org/onto/prop/google_app_engine_flexible_app_version_operating_system">
    <rdfs:label>operating_system</rdfs:label>
    <rdfs:comment>Operating System of the application runtime.</rdfs:comment>
    <rdfs:domain rdf:resource="http://example.org/onto/class/google_app_engine_flexible_app_version"/>
    <rdfs:range rdf:resource="http://www.w3.org/2001/XMLSchema#string"/>
  </owl:DatatypeProperty>
  <owl:DatatypeProperty rdf:about="http://example.org/onto/prop/google_app_engine_flexible_app_version_runtime_version">
    <rdfs:label>runtime_version</rdfs:label>
    <rdfs:comment>The runtime version of an App Engine flexible application.</rdfs:comment>
    <rdfs:domain rdf:resource="http://example.org/onto/class/google_app_engine_flexible_app_version"/>
    <rdfs:range rdf:resource="http://www.w3.org/2001/XMLSchema#string"/>
  </owl:DatatypeProperty>
  <owl:DatatypeProperty rdf:about="http://example.org/onto/prop/google_app_engine_flexible_app_version_auth_fail_action">
    <rdfs:label>auth_fail_action</rdfs:label>
    <rdfs:comment>Actions to take when the user is not logged in. Possible values: ["AUTH_FAIL_ACTION_REDIRECT", "AUTH_FAIL_ACTION_UNAUTHORIZED"]</rdfs:comment>
    <rdfs:domain rdf:resource="http://example.org/onto/class/google_app_engine_flexible_app_version"/>
    <rdfs:range rdf:resource="http://www.w3.org/2001/XMLSchema#string"/>
  </owl:DatatypeProperty>
  <owl:DatatypeProperty rdf:about="http://example.org/onto/prop/google_app_engine_flexible_app_version_login">
    <rdfs:label>login</rdfs:label>
    <rdfs:comment>Methods to restrict access to a URL based on login status. Possible values: ["LOGIN_OPTIONAL", "LOGIN_ADMIN", "LOGIN_REQUIRED"]</rdfs:comment>
    <rdfs:domain rdf:resource="http://example.org/onto/class/google_app_engine_flexible_app_version"/>
    <rdfs:range rdf:resource="http://www.w3.org/2001/XMLSchema#string"/>
  </owl:DatatypeProperty>
  <owl:DatatypeProperty rdf:about="http://example.org/onto/prop/google_app_engine_flexible_app_version_redirect_http_response_code">
    <rdfs:label>redirect_http_response_code</rdfs:label>
    <rdfs:comment>30x code to use when performing redirects for the secure field. Possible values: ["REDIRECT_HTTP_RESPONSE_CODE_301", "REDIRECT_HTTP_RESPONSE_CODE_302", "REDIRECT_HTTP_RESPONSE_CODE_303", "REDIRECT_HTTP_RESPONSE_CODE_307"]</rdfs:comment>
    <rdfs:domain rdf:resource="http://example.org/onto/class/google_app_engine_flexible_app_version"/>
    <rdfs:range rdf:resource="http://www.w3.org/2001/XMLSchema#string"/>
  </owl:DatatypeProperty>
  <owl:DatatypeProperty rdf:about="http://example.org/onto/prop/google_app_engine_flexible_app_version_security_level">
    <rdfs:label>security_level</rdfs:label>
    <rdfs:comment>Security (HTTPS) enforcement for this URL. Possible values: ["SECURE_DEFAULT", "SECURE_NEVER", "SECURE_OPTIONAL", "SECURE_ALWAYS"]</rdfs:comment>
    <rdfs:domain rdf:resource="http://example.org/onto/class/google_app_engine_flexible_app_version"/>
    <rdfs:range rdf:resource="http://www.w3.org/2001/XMLSchema#string"/>
  </owl:DatatypeProperty>
  <owl:DatatypeProperty rdf:about="http://example.org/onto/prop/google_app_engine_flexible_app_version_url_regex">
    <rdfs:label>url_regex</rdfs:label>
    <rdfs:comment>URL prefix. Uses regular expression syntax, which means regexp special characters must be escaped, but should not contain groupings.
All URLs that begin with this prefix are handled by this handler, using the portion of the URL after the prefix as part of the file path.</rdfs:comment>
    <rdfs:domain rdf:resource="http://example.org/onto/class/google_app_engine_flexible_app_version"/>
    <rdfs:range rdf:resource="http://www.w3.org/2001/XMLSchema#string"/>
  </owl:DatatypeProperty>
  <owl:DatatypeProperty rdf:about="http://example.org/onto/prop/google_app_engine_flexible_app_version_script_path">
    <rdfs:label>script_path</rdfs:label>
    <rdfs:comment>Path to the script from the application root directory.</rdfs:comment>
    <rdfs:domain rdf:resource="http://example.org/onto/class/google_app_engine_flexible_app_version"/>
    <rdfs:range rdf:resource="http://www.w3.org/2001/XMLSchema#string"/>
  </owl:DatatypeProperty>
  <owl:DatatypeProperty rdf:about="http://example.org/onto/prop/google_app_engine_flexible_app_version_application_readable">
    <rdfs:label>application_readable</rdfs:label>
    <rdfs:comment>Whether files should also be uploaded as code data. By default, files declared in static file handlers are
uploaded as static data and are only served to end users; they cannot be read by the application. If enabled,
uploads are charged against both your code and static data storage resource quotas.</rdfs:comment>
    <rdfs:domain rdf:resource="http://example.org/onto/class/google_app_engine_flexible_app_version"/>
    <rdfs:range rdf:resource="http://www.w3.org/2001/XMLSchema#string"/>
  </owl:DatatypeProperty>
  <owl:DatatypeProperty rdf:about="http://example.org/onto/prop/google_app_engine_flexible_app_version_expiration">
    <rdfs:label>expiration</rdfs:label>
    <rdfs:comment>Time a static file served by this handler should be cached by web proxies and browsers.
A duration in seconds with up to nine fractional digits, terminated by 's'. Example "3.5s".
Default is '0s'</rdfs:comment>
    <rdfs:domain rdf:resource="http://example.org/onto/class/google_app_engine_flexible_app_version"/>
    <rdfs:range rdf:resource="http://www.w3.org/2001/XMLSchema#string"/>
  </owl:DatatypeProperty>
  <owl:DatatypeProperty rdf:about="http://example.org/onto/prop/google_app_engine_flexible_app_version_http_headers">
    <rdfs:label>http_headers</rdfs:label>
    <rdfs:comment>HTTP headers to use for all responses from these URLs.
An object containing a list of "key:value" value pairs.".</rdfs:comment>
    <rdfs:domain rdf:resource="http://example.org/onto/class/google_app_engine_flexible_app_version"/>
    <rdfs:range rdf:resource="http://www.w3.org/2001/XMLSchema#string"/>
  </owl:DatatypeProperty>
  <owl:DatatypeProperty rdf:about="http://example.org/onto/prop/google_app_engine_flexible_app_version_mime_type">
    <rdfs:label>mime_type</rdfs:label>
    <rdfs:comment>MIME type used to serve all files served by this handler.
Defaults to file-specific MIME types, which are derived from each file's filename extension.</rdfs:comment>
    <rdfs:domain rdf:resource="http://example.org/onto/class/google_app_engine_flexible_app_version"/>
    <rdfs:range rdf:resource="http://www.w3.org/2001/XMLSchema#string"/>
  </owl:DatatypeProperty>
  <owl:DatatypeProperty rdf:about="http://example.org/onto/prop/google_app_engine_flexible_app_version_path">
    <rdfs:label>path</rdfs:label>
    <rdfs:comment>Path to the static files matched by the URL pattern, from the application root directory.
The path can refer to text matched in groupings in the URL pattern.</rdfs:comment>
    <rdfs:domain rdf:resource="http://example.org/onto/class/google_app_engine_flexible_app_version"/>
    <rdfs:range rdf:resource="http://www.w3.org/2001/XMLSchema#string"/>
  </owl:DatatypeProperty>
  <owl:DatatypeProperty rdf:about="http://example.org/onto/prop/google_app_engine_flexible_app_version_require_matching_file">
    <rdfs:label>require_matching_file</rdfs:label>
    <rdfs:comment>Whether this handler should match the request if the file referenced by the handler does not exist.</rdfs:comment>
    <rdfs:domain rdf:resource="http://example.org/onto/class/google_app_engine_flexible_app_version"/>
    <rdfs:range rdf:resource="http://www.w3.org/2001/XMLSchema#string"/>
  </owl:DatatypeProperty>
  <owl:DatatypeProperty rdf:about="http://example.org/onto/prop/google_app_engine_flexible_app_version_upload_path_regex">
    <rdfs:label>upload_path_regex</rdfs:label>
    <rdfs:comment>Regular expression that matches the file paths for all files that should be referenced by this handler.</rdfs:comment>
    <rdfs:domain rdf:resource="http://example.org/onto/class/google_app_engine_flexible_app_version"/>
    <rdfs:range rdf:resource="http://www.w3.org/2001/XMLSchema#string"/>
  </owl:DatatypeProperty>
  <owl:DatatypeProperty rdf:about="http://example.org/onto/prop/google_app_engine_flexible_app_version_check_interval">
    <rdfs:label>check_interval</rdfs:label>
    <rdfs:comment>Interval between health checks.</rdfs:comment>
    <rdfs:domain rdf:resource="http://example.org/onto/class/google_app_engine_flexible_app_version"/>
    <rdfs:range rdf:resource="http://www.w3.org/2001/XMLSchema#string"/>
  </owl:DatatypeProperty>
  <owl:DatatypeProperty rdf:about="http://example.org/onto/prop/google_app_engine_flexible_app_version_failure_threshold">
    <rdfs:label>failure_threshold</rdfs:label>
    <rdfs:comment>Number of consecutive failed checks required before considering the VM unhealthy. Default: 4.</rdfs:comment>
    <rdfs:domain rdf:resource="http://example.org/onto/class/google_app_engine_flexible_app_version"/>
    <rdfs:range rdf:resource="http://www.w3.org/2001/XMLSchema#string"/>
  </owl:DatatypeProperty>
  <owl:DatatypeProperty rdf:about="http://example.org/onto/prop/google_app_engine_flexible_app_version_host">
    <rdfs:label>host</rdfs:label>
    <rdfs:comment>Host header to send when performing a HTTP Readiness check. Example: "myapp.appspot.com"</rdfs:comment>
    <rdfs:domain rdf:resource="http://example.org/onto/class/google_app_engine_flexible_app_version"/>
    <rdfs:range rdf:resource="http://www.w3.org/2001/XMLSchema#string"/>
  </owl:DatatypeProperty>
  <owl:DatatypeProperty rdf:about="http://example.org/onto/prop/google_app_engine_flexible_app_version_initial_delay">
    <rdfs:label>initial_delay</rdfs:label>
    <rdfs:comment>The initial delay before starting to execute the checks. Default: "300s"</rdfs:comment>
    <rdfs:domain rdf:resource="http://example.org/onto/class/google_app_engine_flexible_app_version"/>
    <rdfs:range rdf:resource="http://www.w3.org/2001/XMLSchema#string"/>
  </owl:DatatypeProperty>
  <owl:DatatypeProperty rdf:about="http://example.org/onto/prop/google_app_engine_flexible_app_version_path">
    <rdfs:label>path</rdfs:label>
    <rdfs:comment>The request path.</rdfs:comment>
    <rdfs:domain rdf:resource="http://example.org/onto/class/google_app_engine_flexible_app_version"/>
    <rdfs:range rdf:resource="http://www.w3.org/2001/XMLSchema#string"/>
  </owl:DatatypeProperty>
  <owl:DatatypeProperty rdf:about="http://example.org/onto/prop/google_app_engine_flexible_app_version_success_threshold">
    <rdfs:label>success_threshold</rdfs:label>
    <rdfs:comment>Number of consecutive successful checks required before considering the VM healthy. Default: 2.</rdfs:comment>
    <rdfs:domain rdf:resource="http://example.org/onto/class/google_app_engine_flexible_app_version"/>
    <rdfs:range rdf:resource="http://www.w3.org/2001/XMLSchema#string"/>
  </owl:DatatypeProperty>
  <owl:DatatypeProperty rdf:about="http://example.org/onto/prop/google_app_engine_flexible_app_version_timeout">
    <rdfs:label>timeout</rdfs:label>
    <rdfs:comment>Time before the check is considered failed. Default: "4s"</rdfs:comment>
    <rdfs:domain rdf:resource="http://example.org/onto/class/google_app_engine_flexible_app_version"/>
    <rdfs:range rdf:resource="http://www.w3.org/2001/XMLSchema#string"/>
  </owl:DatatypeProperty>
  <owl:DatatypeProperty rdf:about="http://example.org/onto/prop/google_app_engine_flexible_app_version_instances">
    <rdfs:label>instances</rdfs:label>
    <rdfs:comment>Number of instances to assign to the service at the start.

**Note:** When managing the number of instances at runtime through the App Engine Admin API or the (now deprecated) Python 2
Modules API set_num_instances() you must use 'lifecycle.ignore_changes = ["manual_scaling"[0].instances]' to prevent drift detection.</rdfs:comment>
    <rdfs:domain rdf:resource="http://example.org/onto/class/google_app_engine_flexible_app_version"/>
    <rdfs:range rdf:resource="http://www.w3.org/2001/XMLSchema#string"/>
  </owl:DatatypeProperty>
  <owl:DatatypeProperty rdf:about="http://example.org/onto/prop/google_app_engine_flexible_app_version_forwarded_ports">
    <rdfs:label>forwarded_ports</rdfs:label>
    <rdfs:comment>List of ports, or port pairs, to forward from the virtual machine to the application container.</rdfs:comment>
    <rdfs:domain rdf:resource="http://example.org/onto/class/google_app_engine_flexible_app_version"/>
    <rdfs:range rdf:resource="http://www.w3.org/2001/XMLSchema#string"/>
  </owl:DatatypeProperty>
  <owl:DatatypeProperty rdf:about="http://example.org/onto/prop/google_app_engine_flexible_app_version_instance_tag">
    <rdfs:label>instance_tag</rdfs:label>
    <rdfs:comment>Tag to apply to the instance during creation.</rdfs:comment>
    <rdfs:domain rdf:resource="http://example.org/onto/class/google_app_engine_flexible_app_version"/>
    <rdfs:range rdf:resource="http://www.w3.org/2001/XMLSchema#string"/>
  </owl:DatatypeProperty>
  <owl:DatatypeProperty rdf:about="http://example.org/onto/prop/google_app_engine_flexible_app_version_name">
    <rdfs:label>name</rdfs:label>
    <rdfs:comment>Google Compute Engine network where the virtual machines are created. Specify the short name, not the resource path.</rdfs:comment>
    <rdfs:domain rdf:resource="http://example.org/onto/class/google_app_engine_flexible_app_version"/>
    <rdfs:range rdf:resource="http://www.w3.org/2001/XMLSchema#string"/>
  </owl:DatatypeProperty>
  <owl:DatatypeProperty rdf:about="http://example.org/onto/prop/google_app_engine_flexible_app_version_session_affinity">
    <rdfs:label>session_affinity</rdfs:label>
    <rdfs:comment>Enable session affinity.</rdfs:comment>
    <rdfs:domain rdf:resource="http://example.org/onto/class/google_app_engine_flexible_app_version"/>
    <rdfs:range rdf:resource="http://www.w3.org/2001/XMLSchema#string"/>
  </owl:DatatypeProperty>
  <owl:DatatypeProperty rdf:about="http://example.org/onto/prop/google_app_engine_flexible_app_version_subnetwork">
    <rdfs:label>subnetwork</rdfs:label>
    <rdfs:comment>Google Cloud Platform sub-network where the virtual machines are created. Specify the short name, not the resource path.

If the network that the instance is being created in is a Legacy network, then the IP address is allocated from the IPv4Range.
If the network that the instance is being created in is an auto Subnet Mode Network, then only network name should be specified (not the subnetworkName) and the IP address is created from the IPCidrRange of the subnetwork that exists in that zone for that network.
If the network that the instance is being created in is a custom Subnet Mode Network, then the subnetworkName must be specified and the IP address is created from the IPCidrRange of the subnetwork.
If specified, the subnetwork must exist in the same region as the App Engine flexible environment application.</rdfs:comment>
    <rdfs:domain rdf:resource="http://example.org/onto/class/google_app_engine_flexible_app_version"/>
    <rdfs:range rdf:resource="http://www.w3.org/2001/XMLSchema#string"/>
  </owl:DatatypeProperty>
  <owl:DatatypeProperty rdf:about="http://example.org/onto/prop/google_app_engine_flexible_app_version_app_start_timeout">
    <rdfs:label>app_start_timeout</rdfs:label>
    <rdfs:comment>A maximum time limit on application initialization, measured from moment the application successfully
replies to a healthcheck until it is ready to serve traffic. Default: "300s"</rdfs:comment>
    <rdfs:domain rdf:resource="http://example.org/onto/class/google_app_engine_flexible_app_version"/>
    <rdfs:range rdf:resource="http://www.w3.org/2001/XMLSchema#string"/>
  </owl:DatatypeProperty>
  <owl:DatatypeProperty rdf:about="http://example.org/onto/prop/google_app_engine_flexible_app_version_check_interval">
    <rdfs:label>check_interval</rdfs:label>
    <rdfs:comment>Interval between health checks.  Default: "5s".</rdfs:comment>
    <rdfs:domain rdf:resource="http://example.org/onto/class/google_app_engine_flexible_app_version"/>
    <rdfs:range rdf:resource="http://www.w3.org/2001/XMLSchema#string"/>
  </owl:DatatypeProperty>
  <owl:DatatypeProperty rdf:about="http://example.org/onto/prop/google_app_engine_flexible_app_version_failure_threshold">
    <rdfs:label>failure_threshold</rdfs:label>
    <rdfs:comment>Number of consecutive failed checks required before removing traffic. Default: 2.</rdfs:comment>
    <rdfs:domain rdf:resource="http://example.org/onto/class/google_app_engine_flexible_app_version"/>
    <rdfs:range rdf:resource="http://www.w3.org/2001/XMLSchema#string"/>
  </owl:DatatypeProperty>
  <owl:DatatypeProperty rdf:about="http://example.org/onto/prop/google_app_engine_flexible_app_version_host">
    <rdfs:label>host</rdfs:label>
    <rdfs:comment>Host header to send when performing a HTTP Readiness check. Example: "myapp.appspot.com"</rdfs:comment>
    <rdfs:domain rdf:resource="http://example.org/onto/class/google_app_engine_flexible_app_version"/>
    <rdfs:range rdf:resource="http://www.w3.org/2001/XMLSchema#string"/>
  </owl:DatatypeProperty>
  <owl:DatatypeProperty rdf:about="http://example.org/onto/prop/google_app_engine_flexible_app_version_path">
    <rdfs:label>path</rdfs:label>
    <rdfs:comment>The request path.</rdfs:comment>
    <rdfs:domain rdf:resource="http://example.org/onto/class/google_app_engine_flexible_app_version"/>
    <rdfs:range rdf:resource="http://www.w3.org/2001/XMLSchema#string"/>
  </owl:DatatypeProperty>
  <owl:DatatypeProperty rdf:about="http://example.org/onto/prop/google_app_engine_flexible_app_version_success_threshold">
    <rdfs:label>success_threshold</rdfs:label>
    <rdfs:comment>Number of consecutive successful checks required before receiving traffic. Default: 2.</rdfs:comment>
    <rdfs:domain rdf:resource="http://example.org/onto/class/google_app_engine_flexible_app_version"/>
    <rdfs:range rdf:resource="http://www.w3.org/2001/XMLSchema#string"/>
  </owl:DatatypeProperty>
  <owl:DatatypeProperty rdf:about="http://example.org/onto/prop/google_app_engine_flexible_app_version_timeout">
    <rdfs:label>timeout</rdfs:label>
    <rdfs:comment>Time before the check is considered failed. Default: "4s"</rdfs:comment>
    <rdfs:domain rdf:resource="http://example.org/onto/class/google_app_engine_flexible_app_version"/>
    <rdfs:range rdf:resource="http://www.w3.org/2001/XMLSchema#string"/>
  </owl:DatatypeProperty>
  <owl:DatatypeProperty rdf:about="http://example.org/onto/prop/google_app_engine_flexible_app_version_cpu">
    <rdfs:label>cpu</rdfs:label>
    <rdfs:comment>Number of CPU cores needed.</rdfs:comment>
    <rdfs:domain rdf:resource="http://example.org/onto/class/google_app_engine_flexible_app_version"/>
    <rdfs:range rdf:resource="http://www.w3.org/2001/XMLSchema#string"/>
  </owl:DatatypeProperty>
  <owl:DatatypeProperty rdf:about="http://example.org/onto/prop/google_app_engine_flexible_app_version_disk_gb">
    <rdfs:label>disk_gb</rdfs:label>
    <rdfs:comment>Disk size (GB) needed.</rdfs:comment>
    <rdfs:domain rdf:resource="http://example.org/onto/class/google_app_engine_flexible_app_version"/>
    <rdfs:range rdf:resource="http://www.w3.org/2001/XMLSchema#string"/>
  </owl:DatatypeProperty>
  <owl:DatatypeProperty rdf:about="http://example.org/onto/prop/google_app_engine_flexible_app_version_memory_gb">
    <rdfs:label>memory_gb</rdfs:label>
    <rdfs:comment>Memory (GB) needed.</rdfs:comment>
    <rdfs:domain rdf:resource="http://example.org/onto/class/google_app_engine_flexible_app_version"/>
    <rdfs:range rdf:resource="http://www.w3.org/2001/XMLSchema#string"/>
  </owl:DatatypeProperty>
  <owl:DatatypeProperty rdf:about="http://example.org/onto/prop/google_app_engine_flexible_app_version_name">
    <rdfs:label>name</rdfs:label>
    <rdfs:comment>Unique name for the volume.</rdfs:comment>
    <rdfs:domain rdf:resource="http://example.org/onto/class/google_app_engine_flexible_app_version"/>
    <rdfs:range rdf:resource="http://www.w3.org/2001/XMLSchema#string"/>
  </owl:DatatypeProperty>
  <owl:DatatypeProperty rdf:about="http://example.org/onto/prop/google_app_engine_flexible_app_version_size_gb">
    <rdfs:label>size_gb</rdfs:label>
    <rdfs:comment>Volume size in gigabytes.</rdfs:comment>
    <rdfs:domain rdf:resource="http://example.org/onto/class/google_app_engine_flexible_app_version"/>
    <rdfs:range rdf:resource="http://www.w3.org/2001/XMLSchema#string"/>
  </owl:DatatypeProperty>
  <owl:DatatypeProperty rdf:about="http://example.org/onto/prop/google_app_engine_flexible_app_version_volume_type">
    <rdfs:label>volume_type</rdfs:label>
    <rdfs:comment>Underlying volume type, e.g. 'tmpfs'.</rdfs:comment>
    <rdfs:domain rdf:resource="http://example.org/onto/class/google_app_engine_flexible_app_version"/>
    <rdfs:range rdf:resource="http://www.w3.org/2001/XMLSchema#string"/>
  </owl:DatatypeProperty>
  <owl:DatatypeProperty rdf:about="http://example.org/onto/prop/google_app_engine_flexible_app_version_create">
    <rdfs:label>create</rdfs:label>
    <rdfs:domain rdf:resource="http://example.org/onto/class/google_app_engine_flexible_app_version"/>
    <rdfs:range rdf:resource="http://www.w3.org/2001/XMLSchema#string"/>
  </owl:DatatypeProperty>
  <owl:DatatypeProperty rdf:about="http://example.org/onto/prop/google_app_engine_flexible_app_version_delete">
    <rdfs:label>delete</rdfs:label>
    <rdfs:domain rdf:resource="http://example.org/onto/class/google_app_engine_flexible_app_version"/>
    <rdfs:range rdf:resource="http://www.w3.org/2001/XMLSchema#string"/>
  </owl:DatatypeProperty>
  <owl:DatatypeProperty rdf:about="http://example.org/onto/prop/google_app_engine_flexible_app_version_update">
    <rdfs:label>update</rdfs:label>
    <rdfs:domain rdf:resource="http://example.org/onto/class/google_app_engine_flexible_app_version"/>
    <rdfs:range rdf:resource="http://www.w3.org/2001/XMLSchema#string"/>
  </owl:DatatypeProperty>
  <owl:DatatypeProperty rdf:about="http://example.org/onto/prop/google_app_engine_flexible_app_version_name">
    <rdfs:label>name</rdfs:label>
    <rdfs:comment>Full Serverless VPC Access Connector name e.g. /projects/my-project/locations/us-central1/connectors/c1.</rdfs:comment>
    <rdfs:domain rdf:resource="http://example.org/onto/class/google_app_engine_flexible_app_version"/>
    <rdfs:range rdf:resource="http://www.w3.org/2001/XMLSchema#string"/>
  </owl:DatatypeProperty>
</rdf:RDF>
