<?xml version="1.0" encoding="UTF-8"?>
<rdf:RDF
  xmlns:rdf="http://www.w3.org/1999/02/22-rdf-syntax-ns#"
  xmlns:rdfs="http://www.w3.org/2000/01/rdf-schema#"
  xmlns:owl="http://www.w3.org/2002/07/owl#"
  xmlns:xsd="http://www.w3.org/2001/XMLSchema#"
  xml:base="http://example.org/onto/">
  <owl:Class rdf:about="http://example.org/onto/class/google_netapp_volume_replication">
    <rdfs:label>google_netapp_volume_replication</rdfs:label>
    <rdfs:comment>#
#     ***     AUTO GENERATED CODE    ***    Type: MMv1     ***
#
# ----------------------------------------------------------------------------
#
#     This code is generated by Magic Modules using the following:
#
#     Configuration: https:#github.com/GoogleCloudPlatform/magic-modules/tree/main/mmv1/products/netapp/VolumeReplication.yaml
#     Template:      https:#github.com/GoogleCloudPlatform/magic-modules/tree/main/mmv1/templates/terraform/resource.html.markdown.tmpl
#
#     DO NOT EDIT this file directly. Any changes made to this file will be
#     overwritten during the next generation cycle.
#
# ----------------------------------------------------------------------------
subcategory: "Google Cloud NetApp Volumes"
description: |-
  Volume replication creates an asynchronous mirror of a volume in a different location.
---</rdfs:comment>
  </owl:Class>
  <owl:DatatypeProperty rdf:about="http://example.org/onto/prop/google_netapp_volume_replication_create_time">
    <rdfs:label>create_time</rdfs:label>
    <rdfs:comment>Create time of the active directory. A timestamp in RFC3339 UTC "Zulu" format. Examples: "2023-06-22T09:13:01.617Z".</rdfs:comment>
    <rdfs:domain rdf:resource="http://example.org/onto/class/google_netapp_volume_replication"/>
    <rdfs:range rdf:resource="http://www.w3.org/2001/XMLSchema#string"/>
  </owl:DatatypeProperty>
  <owl:DatatypeProperty rdf:about="http://example.org/onto/prop/google_netapp_volume_replication_delete_destination_volume">
    <rdfs:label>delete_destination_volume</rdfs:label>
    <rdfs:comment>A destination volume is created as part of replication creation. The destination volume will not became
under Terraform management unless you import it manually. If you delete the replication, this volume
will remain.
Setting this parameter to true will delete the *current* destination volume when destroying the
replication. If you reversed the replication direction, this will be your former source volume!
For production use, it is recommended to keep this parameter false to avoid accidental volume
deletion. Handle with care. Default is false.</rdfs:comment>
    <rdfs:domain rdf:resource="http://example.org/onto/class/google_netapp_volume_replication"/>
    <rdfs:range rdf:resource="http://www.w3.org/2001/XMLSchema#string"/>
  </owl:DatatypeProperty>
  <owl:DatatypeProperty rdf:about="http://example.org/onto/prop/google_netapp_volume_replication_description">
    <rdfs:label>description</rdfs:label>
    <rdfs:comment>An description of this resource.</rdfs:comment>
    <rdfs:domain rdf:resource="http://example.org/onto/class/google_netapp_volume_replication"/>
    <rdfs:range rdf:resource="http://www.w3.org/2001/XMLSchema#string"/>
  </owl:DatatypeProperty>
  <owl:DatatypeProperty rdf:about="http://example.org/onto/prop/google_netapp_volume_replication_destination_volume">
    <rdfs:label>destination_volume</rdfs:label>
    <rdfs:comment>Full resource name of destination volume with format: 'projects/{{project}}/locations/{{location}}/volumes/{{volumeId}}'</rdfs:comment>
    <rdfs:domain rdf:resource="http://example.org/onto/class/google_netapp_volume_replication"/>
    <rdfs:range rdf:resource="http://www.w3.org/2001/XMLSchema#string"/>
  </owl:DatatypeProperty>
  <owl:DatatypeProperty rdf:about="http://example.org/onto/prop/google_netapp_volume_replication_effective_labels">
    <rdfs:label>effective_labels</rdfs:label>
    <rdfs:comment>All of labels (key/value pairs) present on the resource in GCP, including the labels configured through Terraform, other clients and services.</rdfs:comment>
    <rdfs:domain rdf:resource="http://example.org/onto/class/google_netapp_volume_replication"/>
    <rdfs:range rdf:resource="http://www.w3.org/2001/XMLSchema#string"/>
  </owl:DatatypeProperty>
  <owl:DatatypeProperty rdf:about="http://example.org/onto/prop/google_netapp_volume_replication_force_stopping">
    <rdfs:label>force_stopping</rdfs:label>
    <rdfs:comment>Only replications with mirror_state=MIRRORED can be stopped. A replication in mirror_state=TRANSFERRING
currently receives an update and stopping the update might be undesirable. Set this parameter to true
to stop anyway. All data transferred to the destination will be discarded and content of destination
volume will remain at the state of the last successful update. Default is false.</rdfs:comment>
    <rdfs:domain rdf:resource="http://example.org/onto/class/google_netapp_volume_replication"/>
    <rdfs:range rdf:resource="http://www.w3.org/2001/XMLSchema#string"/>
  </owl:DatatypeProperty>
  <owl:DatatypeProperty rdf:about="http://example.org/onto/prop/google_netapp_volume_replication_healthy">
    <rdfs:label>healthy</rdfs:label>
    <rdfs:comment>Condition of the relationship. Can be one of the following:
  - true: The replication relationship is healthy. It has not missed the most recent scheduled transfer.
  - false: The replication relationship is not healthy. It has missed the most recent scheduled transfer.</rdfs:comment>
    <rdfs:domain rdf:resource="http://example.org/onto/class/google_netapp_volume_replication"/>
    <rdfs:range rdf:resource="http://www.w3.org/2001/XMLSchema#string"/>
  </owl:DatatypeProperty>
  <owl:DatatypeProperty rdf:about="http://example.org/onto/prop/google_netapp_volume_replication_hybrid_peering_details">
    <rdfs:label>hybrid_peering_details</rdfs:label>
    <rdfs:comment>HybridPeeringDetails contains details about the hybrid peering.</rdfs:comment>
    <rdfs:domain rdf:resource="http://example.org/onto/class/google_netapp_volume_replication"/>
    <rdfs:range rdf:resource="http://www.w3.org/2001/XMLSchema#string"/>
  </owl:DatatypeProperty>
  <owl:DatatypeProperty rdf:about="http://example.org/onto/prop/google_netapp_volume_replication_hybrid_replication_type">
    <rdfs:label>hybrid_replication_type</rdfs:label>
    <rdfs:comment>Hybrid replication type.</rdfs:comment>
    <rdfs:domain rdf:resource="http://example.org/onto/class/google_netapp_volume_replication"/>
    <rdfs:range rdf:resource="http://www.w3.org/2001/XMLSchema#string"/>
  </owl:DatatypeProperty>
  <owl:DatatypeProperty rdf:about="http://example.org/onto/prop/google_netapp_volume_replication_hybrid_replication_user_commands">
    <rdfs:label>hybrid_replication_user_commands</rdfs:label>
    <rdfs:comment>Copy pastable snapmirror commands to be executed on onprem cluster by the customer.</rdfs:comment>
    <rdfs:domain rdf:resource="http://example.org/onto/class/google_netapp_volume_replication"/>
    <rdfs:range rdf:resource="http://www.w3.org/2001/XMLSchema#string"/>
  </owl:DatatypeProperty>
  <owl:DatatypeProperty rdf:about="http://example.org/onto/prop/google_netapp_volume_replication_id">
    <rdfs:label>id</rdfs:label>
    <rdfs:domain rdf:resource="http://example.org/onto/class/google_netapp_volume_replication"/>
    <rdfs:range rdf:resource="http://www.w3.org/2001/XMLSchema#string"/>
  </owl:DatatypeProperty>
  <owl:DatatypeProperty rdf:about="http://example.org/onto/prop/google_netapp_volume_replication_labels">
    <rdfs:label>labels</rdfs:label>
    <rdfs:comment>Labels as key value pairs. Example: '{ "owner": "Bob", "department": "finance", "purpose": "testing" }'


**Note**: This field is non-authoritative, and will only manage the labels present in your configuration.
Please refer to the field 'effective_labels' for all of the labels present on the resource.</rdfs:comment>
    <rdfs:domain rdf:resource="http://example.org/onto/class/google_netapp_volume_replication"/>
    <rdfs:range rdf:resource="http://www.w3.org/2001/XMLSchema#string"/>
  </owl:DatatypeProperty>
  <owl:DatatypeProperty rdf:about="http://example.org/onto/prop/google_netapp_volume_replication_location">
    <rdfs:label>location</rdfs:label>
    <rdfs:comment>Name of region for this resource. The resource needs to be created in the region of the destination volume.</rdfs:comment>
    <rdfs:domain rdf:resource="http://example.org/onto/class/google_netapp_volume_replication"/>
    <rdfs:range rdf:resource="http://www.w3.org/2001/XMLSchema#string"/>
  </owl:DatatypeProperty>
  <owl:DatatypeProperty rdf:about="http://example.org/onto/prop/google_netapp_volume_replication_mirror_state">
    <rdfs:label>mirror_state</rdfs:label>
    <rdfs:comment>Indicates the state of the mirror between source and destination volumes. Depending on the amount of data
in your source volume, PREPARING phase can take hours or days. mirrorState = MIRRORED indicates your baseline
transfer ended and destination volume became accessible read-only. TRANSFERRING means a MIRRORED volume
currently receives an update. Updated every 5 minutes.</rdfs:comment>
    <rdfs:domain rdf:resource="http://example.org/onto/class/google_netapp_volume_replication"/>
    <rdfs:range rdf:resource="http://www.w3.org/2001/XMLSchema#string"/>
  </owl:DatatypeProperty>
  <owl:DatatypeProperty rdf:about="http://example.org/onto/prop/google_netapp_volume_replication_name">
    <rdfs:label>name</rdfs:label>
    <rdfs:comment>The name of the replication. Needs to be unique per location.</rdfs:comment>
    <rdfs:domain rdf:resource="http://example.org/onto/class/google_netapp_volume_replication"/>
    <rdfs:range rdf:resource="http://www.w3.org/2001/XMLSchema#string"/>
  </owl:DatatypeProperty>
  <owl:DatatypeProperty rdf:about="http://example.org/onto/prop/google_netapp_volume_replication_project">
    <rdfs:label>project</rdfs:label>
    <rdfs:domain rdf:resource="http://example.org/onto/class/google_netapp_volume_replication"/>
    <rdfs:range rdf:resource="http://www.w3.org/2001/XMLSchema#string"/>
  </owl:DatatypeProperty>
  <owl:DatatypeProperty rdf:about="http://example.org/onto/prop/google_netapp_volume_replication_replication_enabled">
    <rdfs:label>replication_enabled</rdfs:label>
    <rdfs:comment>Set to false to stop/break the mirror. Stopping the mirror makes the destination volume read-write
and act independently from the source volume.
Set to true to enable/resume the mirror. WARNING: Resuming a mirror overwrites any changes
done to the destination volume with the content of the source volume.</rdfs:comment>
    <rdfs:domain rdf:resource="http://example.org/onto/class/google_netapp_volume_replication"/>
    <rdfs:range rdf:resource="http://www.w3.org/2001/XMLSchema#string"/>
  </owl:DatatypeProperty>
  <owl:DatatypeProperty rdf:about="http://example.org/onto/prop/google_netapp_volume_replication_replication_schedule">
    <rdfs:label>replication_schedule</rdfs:label>
    <rdfs:comment>Specifies the replication interval. Possible values: ["EVERY_10_MINUTES", "HOURLY", "DAILY"]</rdfs:comment>
    <rdfs:domain rdf:resource="http://example.org/onto/class/google_netapp_volume_replication"/>
    <rdfs:range rdf:resource="http://www.w3.org/2001/XMLSchema#string"/>
  </owl:DatatypeProperty>
  <owl:DatatypeProperty rdf:about="http://example.org/onto/prop/google_netapp_volume_replication_role">
    <rdfs:label>role</rdfs:label>
    <rdfs:comment>Reverting a replication can swap source and destination volume roles. This field indicates if the 'location' hosts
the source or destination volume. For resume and revert and resume operations it is critical to understand
which volume is the source volume, since it will overwrite changes done to the destination volume.</rdfs:comment>
    <rdfs:domain rdf:resource="http://example.org/onto/class/google_netapp_volume_replication"/>
    <rdfs:range rdf:resource="http://www.w3.org/2001/XMLSchema#string"/>
  </owl:DatatypeProperty>
  <owl:DatatypeProperty rdf:about="http://example.org/onto/prop/google_netapp_volume_replication_source_volume">
    <rdfs:label>source_volume</rdfs:label>
    <rdfs:comment>Full resource name of source volume with format: 'projects/{{project}}/locations/{{location}}/volumes/{{volumeId}}'</rdfs:comment>
    <rdfs:domain rdf:resource="http://example.org/onto/class/google_netapp_volume_replication"/>
    <rdfs:range rdf:resource="http://www.w3.org/2001/XMLSchema#string"/>
  </owl:DatatypeProperty>
  <owl:DatatypeProperty rdf:about="http://example.org/onto/prop/google_netapp_volume_replication_state">
    <rdfs:label>state</rdfs:label>
    <rdfs:comment>Indicates the state of replication resource. State of the mirror itself is indicated in mirrorState.</rdfs:comment>
    <rdfs:domain rdf:resource="http://example.org/onto/class/google_netapp_volume_replication"/>
    <rdfs:range rdf:resource="http://www.w3.org/2001/XMLSchema#string"/>
  </owl:DatatypeProperty>
  <owl:DatatypeProperty rdf:about="http://example.org/onto/prop/google_netapp_volume_replication_state_details">
    <rdfs:label>state_details</rdfs:label>
    <rdfs:comment>State details of the replication resource.</rdfs:comment>
    <rdfs:domain rdf:resource="http://example.org/onto/class/google_netapp_volume_replication"/>
    <rdfs:range rdf:resource="http://www.w3.org/2001/XMLSchema#string"/>
  </owl:DatatypeProperty>
  <owl:DatatypeProperty rdf:about="http://example.org/onto/prop/google_netapp_volume_replication_terraform_labels">
    <rdfs:label>terraform_labels</rdfs:label>
    <rdfs:comment>The combination of labels configured directly on the resource
 and default labels configured on the provider.</rdfs:comment>
    <rdfs:domain rdf:resource="http://example.org/onto/class/google_netapp_volume_replication"/>
    <rdfs:range rdf:resource="http://www.w3.org/2001/XMLSchema#string"/>
  </owl:DatatypeProperty>
  <owl:DatatypeProperty rdf:about="http://example.org/onto/prop/google_netapp_volume_replication_transfer_stats">
    <rdfs:label>transfer_stats</rdfs:label>
    <rdfs:comment>Replication transfer statistics. All statistics are updated every 5 minutes.</rdfs:comment>
    <rdfs:domain rdf:resource="http://example.org/onto/class/google_netapp_volume_replication"/>
    <rdfs:range rdf:resource="http://www.w3.org/2001/XMLSchema#string"/>
  </owl:DatatypeProperty>
  <owl:DatatypeProperty rdf:about="http://example.org/onto/prop/google_netapp_volume_replication_volume_name">
    <rdfs:label>volume_name</rdfs:label>
    <rdfs:comment>The name of the existing source volume.</rdfs:comment>
    <rdfs:domain rdf:resource="http://example.org/onto/class/google_netapp_volume_replication"/>
    <rdfs:range rdf:resource="http://www.w3.org/2001/XMLSchema#string"/>
  </owl:DatatypeProperty>
  <owl:DatatypeProperty rdf:about="http://example.org/onto/prop/google_netapp_volume_replication_wait_for_mirror">
    <rdfs:label>wait_for_mirror</rdfs:label>
    <rdfs:comment>Replication resource state is independent of mirror_state. With enough data, it can take many hours
for mirror_state to reach MIRRORED. If you want Terraform to wait for the mirror to finish on
create/stop/resume operations, set this parameter to true. Default is false.</rdfs:comment>
    <rdfs:domain rdf:resource="http://example.org/onto/class/google_netapp_volume_replication"/>
    <rdfs:range rdf:resource="http://www.w3.org/2001/XMLSchema#string"/>
  </owl:DatatypeProperty>
  <owl:DatatypeProperty rdf:about="http://example.org/onto/prop/google_netapp_volume_replication_description">
    <rdfs:label>description</rdfs:label>
    <rdfs:comment>Description for the destination volume.</rdfs:comment>
    <rdfs:domain rdf:resource="http://example.org/onto/class/google_netapp_volume_replication"/>
    <rdfs:range rdf:resource="http://www.w3.org/2001/XMLSchema#string"/>
  </owl:DatatypeProperty>
  <owl:DatatypeProperty rdf:about="http://example.org/onto/prop/google_netapp_volume_replication_share_name">
    <rdfs:label>share_name</rdfs:label>
    <rdfs:comment>Share name for destination volume. If not specified, name of source volume's share name will be used.</rdfs:comment>
    <rdfs:domain rdf:resource="http://example.org/onto/class/google_netapp_volume_replication"/>
    <rdfs:range rdf:resource="http://www.w3.org/2001/XMLSchema#string"/>
  </owl:DatatypeProperty>
  <owl:DatatypeProperty rdf:about="http://example.org/onto/prop/google_netapp_volume_replication_storage_pool">
    <rdfs:label>storage_pool</rdfs:label>
    <rdfs:comment>Name of an existing storage pool for the destination volume with format: 'projects/{{project}}/locations/{{location}}/storagePools/{{poolId}}'</rdfs:comment>
    <rdfs:domain rdf:resource="http://example.org/onto/class/google_netapp_volume_replication"/>
    <rdfs:range rdf:resource="http://www.w3.org/2001/XMLSchema#string"/>
  </owl:DatatypeProperty>
  <owl:DatatypeProperty rdf:about="http://example.org/onto/prop/google_netapp_volume_replication_volume_id">
    <rdfs:label>volume_id</rdfs:label>
    <rdfs:comment>Name for the destination volume to be created. If not specified, the name of the source volume will be used.</rdfs:comment>
    <rdfs:domain rdf:resource="http://example.org/onto/class/google_netapp_volume_replication"/>
    <rdfs:range rdf:resource="http://www.w3.org/2001/XMLSchema#string"/>
  </owl:DatatypeProperty>
  <owl:DatatypeProperty rdf:about="http://example.org/onto/prop/google_netapp_volume_replication_cooling_threshold_days">
    <rdfs:label>cooling_threshold_days</rdfs:label>
    <rdfs:comment>Optional. Time in days to mark the volume's data block as cold and make it eligible for tiering, can be range from 2-183.
Default is 31.</rdfs:comment>
    <rdfs:domain rdf:resource="http://example.org/onto/class/google_netapp_volume_replication"/>
    <rdfs:range rdf:resource="http://www.w3.org/2001/XMLSchema#string"/>
  </owl:DatatypeProperty>
  <owl:DatatypeProperty rdf:about="http://example.org/onto/prop/google_netapp_volume_replication_tier_action">
    <rdfs:label>tier_action</rdfs:label>
    <rdfs:comment>Optional. Flag indicating if the volume has tiering policy enable/pause. Default is PAUSED. Default value: "PAUSED" Possible values: ["ENABLED", "PAUSED"]</rdfs:comment>
    <rdfs:domain rdf:resource="http://example.org/onto/class/google_netapp_volume_replication"/>
    <rdfs:range rdf:resource="http://www.w3.org/2001/XMLSchema#string"/>
  </owl:DatatypeProperty>
  <owl:DatatypeProperty rdf:about="http://example.org/onto/prop/google_netapp_volume_replication_create">
    <rdfs:label>create</rdfs:label>
    <rdfs:domain rdf:resource="http://example.org/onto/class/google_netapp_volume_replication"/>
    <rdfs:range rdf:resource="http://www.w3.org/2001/XMLSchema#string"/>
  </owl:DatatypeProperty>
  <owl:DatatypeProperty rdf:about="http://example.org/onto/prop/google_netapp_volume_replication_delete">
    <rdfs:label>delete</rdfs:label>
    <rdfs:domain rdf:resource="http://example.org/onto/class/google_netapp_volume_replication"/>
    <rdfs:range rdf:resource="http://www.w3.org/2001/XMLSchema#string"/>
  </owl:DatatypeProperty>
  <owl:DatatypeProperty rdf:about="http://example.org/onto/prop/google_netapp_volume_replication_update">
    <rdfs:label>update</rdfs:label>
    <rdfs:domain rdf:resource="http://example.org/onto/class/google_netapp_volume_replication"/>
    <rdfs:range rdf:resource="http://www.w3.org/2001/XMLSchema#string"/>
  </owl:DatatypeProperty>
</rdf:RDF>
