<?xml version="1.0" encoding="UTF-8"?>
<rdf:RDF
  xmlns:rdf="http://www.w3.org/1999/02/22-rdf-syntax-ns#"
  xmlns:rdfs="http://www.w3.org/2000/01/rdf-schema#"
  xmlns:owl="http://www.w3.org/2002/07/owl#"
  xmlns:xsd="http://www.w3.org/2001/XMLSchema#"
  xml:base="http://example.org/onto/">
  <owl:Class rdf:about="http://example.org/onto/class/google_managed_kafka_cluster">
    <rdfs:label>google_managed_kafka_cluster</rdfs:label>
    <rdfs:comment>#
#     ***     AUTO GENERATED CODE    ***    Type: MMv1     ***
#
# ----------------------------------------------------------------------------
#
#     This code is generated by Magic Modules using the following:
#
#     Configuration: https:#github.com/GoogleCloudPlatform/magic-modules/tree/main/mmv1/products/managedkafka/Cluster.yaml
#     Template:      https:#github.com/GoogleCloudPlatform/magic-modules/tree/main/mmv1/templates/terraform/resource.html.markdown.tmpl
#
#     DO NOT EDIT this file directly. Any changes made to this file will be
#     overwritten during the next generation cycle.
#
# ----------------------------------------------------------------------------
subcategory: "Managed Kafka"
description: |-
  A Managed Service for Apache Kafka cluster.
---</rdfs:comment>
  </owl:Class>
  <owl:DatatypeProperty rdf:about="http://example.org/onto/prop/google_managed_kafka_cluster_cluster_id">
    <rdfs:label>cluster_id</rdfs:label>
    <rdfs:comment>The ID to use for the cluster, which will become the final component of the cluster's name. The ID must be 1-63 characters long, and match the regular expression '[a-z]([-a-z0-9]*[a-z0-9])?' to comply with RFC 1035. This value is structured like: 'my-cluster-id'.</rdfs:comment>
    <rdfs:domain rdf:resource="http://example.org/onto/class/google_managed_kafka_cluster"/>
    <rdfs:range rdf:resource="http://www.w3.org/2001/XMLSchema#string"/>
  </owl:DatatypeProperty>
  <owl:DatatypeProperty rdf:about="http://example.org/onto/prop/google_managed_kafka_cluster_create_time">
    <rdfs:label>create_time</rdfs:label>
    <rdfs:comment>The time when the cluster was created.</rdfs:comment>
    <rdfs:domain rdf:resource="http://example.org/onto/class/google_managed_kafka_cluster"/>
    <rdfs:range rdf:resource="http://www.w3.org/2001/XMLSchema#string"/>
  </owl:DatatypeProperty>
  <owl:DatatypeProperty rdf:about="http://example.org/onto/prop/google_managed_kafka_cluster_effective_labels">
    <rdfs:label>effective_labels</rdfs:label>
    <rdfs:comment>All of labels (key/value pairs) present on the resource in GCP, including the labels configured through Terraform, other clients and services.</rdfs:comment>
    <rdfs:domain rdf:resource="http://example.org/onto/class/google_managed_kafka_cluster"/>
    <rdfs:range rdf:resource="http://www.w3.org/2001/XMLSchema#string"/>
  </owl:DatatypeProperty>
  <owl:DatatypeProperty rdf:about="http://example.org/onto/prop/google_managed_kafka_cluster_id">
    <rdfs:label>id</rdfs:label>
    <rdfs:domain rdf:resource="http://example.org/onto/class/google_managed_kafka_cluster"/>
    <rdfs:range rdf:resource="http://www.w3.org/2001/XMLSchema#string"/>
  </owl:DatatypeProperty>
  <owl:DatatypeProperty rdf:about="http://example.org/onto/prop/google_managed_kafka_cluster_labels">
    <rdfs:label>labels</rdfs:label>
    <rdfs:comment>List of label KEY=VALUE pairs to add. Keys must start with a lowercase character and contain only hyphens (-), underscores ( ), lowercase characters, and numbers. Values must contain only hyphens (-), underscores ( ), lowercase characters, and numbers.

**Note**: This field is non-authoritative, and will only manage the labels present in your configuration.
Please refer to the field 'effective_labels' for all of the labels present on the resource.</rdfs:comment>
    <rdfs:domain rdf:resource="http://example.org/onto/class/google_managed_kafka_cluster"/>
    <rdfs:range rdf:resource="http://www.w3.org/2001/XMLSchema#string"/>
  </owl:DatatypeProperty>
  <owl:DatatypeProperty rdf:about="http://example.org/onto/prop/google_managed_kafka_cluster_location">
    <rdfs:label>location</rdfs:label>
    <rdfs:comment>ID of the location of the Kafka resource. See https://cloud.google.com/managed-kafka/docs/locations for a list of supported locations.</rdfs:comment>
    <rdfs:domain rdf:resource="http://example.org/onto/class/google_managed_kafka_cluster"/>
    <rdfs:range rdf:resource="http://www.w3.org/2001/XMLSchema#string"/>
  </owl:DatatypeProperty>
  <owl:DatatypeProperty rdf:about="http://example.org/onto/prop/google_managed_kafka_cluster_name">
    <rdfs:label>name</rdfs:label>
    <rdfs:comment>The name of the cluster. Structured like: 'projects/PROJECT_ID/locations/LOCATION/clusters/CLUSTER_ID'.</rdfs:comment>
    <rdfs:domain rdf:resource="http://example.org/onto/class/google_managed_kafka_cluster"/>
    <rdfs:range rdf:resource="http://www.w3.org/2001/XMLSchema#string"/>
  </owl:DatatypeProperty>
  <owl:DatatypeProperty rdf:about="http://example.org/onto/prop/google_managed_kafka_cluster_project">
    <rdfs:label>project</rdfs:label>
    <rdfs:domain rdf:resource="http://example.org/onto/class/google_managed_kafka_cluster"/>
    <rdfs:range rdf:resource="http://www.w3.org/2001/XMLSchema#string"/>
  </owl:DatatypeProperty>
  <owl:DatatypeProperty rdf:about="http://example.org/onto/prop/google_managed_kafka_cluster_state">
    <rdfs:label>state</rdfs:label>
    <rdfs:comment>The current state of the cluster. Possible values: 'STATE_UNSPECIFIED', 'CREATING', 'ACTIVE', 'DELETING'.</rdfs:comment>
    <rdfs:domain rdf:resource="http://example.org/onto/class/google_managed_kafka_cluster"/>
    <rdfs:range rdf:resource="http://www.w3.org/2001/XMLSchema#string"/>
  </owl:DatatypeProperty>
  <owl:DatatypeProperty rdf:about="http://example.org/onto/prop/google_managed_kafka_cluster_terraform_labels">
    <rdfs:label>terraform_labels</rdfs:label>
    <rdfs:comment>The combination of labels configured directly on the resource
 and default labels configured on the provider.</rdfs:comment>
    <rdfs:domain rdf:resource="http://example.org/onto/class/google_managed_kafka_cluster"/>
    <rdfs:range rdf:resource="http://www.w3.org/2001/XMLSchema#string"/>
  </owl:DatatypeProperty>
  <owl:DatatypeProperty rdf:about="http://example.org/onto/prop/google_managed_kafka_cluster_update_time">
    <rdfs:label>update_time</rdfs:label>
    <rdfs:comment>The time when the cluster was last updated.</rdfs:comment>
    <rdfs:domain rdf:resource="http://example.org/onto/class/google_managed_kafka_cluster"/>
    <rdfs:range rdf:resource="http://www.w3.org/2001/XMLSchema#string"/>
  </owl:DatatypeProperty>
  <owl:DatatypeProperty rdf:about="http://example.org/onto/prop/google_managed_kafka_cluster_memory_bytes">
    <rdfs:label>memory_bytes</rdfs:label>
    <rdfs:comment>The memory to provision for the cluster in bytes. The value must be between 1 GiB and 8 GiB per vCPU. Ex. 1024Mi, 4Gi.</rdfs:comment>
    <rdfs:domain rdf:resource="http://example.org/onto/class/google_managed_kafka_cluster"/>
    <rdfs:range rdf:resource="http://www.w3.org/2001/XMLSchema#string"/>
  </owl:DatatypeProperty>
  <owl:DatatypeProperty rdf:about="http://example.org/onto/prop/google_managed_kafka_cluster_vcpu_count">
    <rdfs:label>vcpu_count</rdfs:label>
    <rdfs:comment>The number of vCPUs to provision for the cluster. The minimum is 3.</rdfs:comment>
    <rdfs:domain rdf:resource="http://example.org/onto/class/google_managed_kafka_cluster"/>
    <rdfs:range rdf:resource="http://www.w3.org/2001/XMLSchema#string"/>
  </owl:DatatypeProperty>
  <owl:DatatypeProperty rdf:about="http://example.org/onto/prop/google_managed_kafka_cluster_kms_key">
    <rdfs:label>kms_key</rdfs:label>
    <rdfs:comment>The Cloud KMS Key name to use for encryption. The key must be located in the same region as the cluster and cannot be changed. Must be in the format 'projects/PROJECT_ID/locations/LOCATION/keyRings/KEY_RING/cryptoKeys/KEY'.</rdfs:comment>
    <rdfs:domain rdf:resource="http://example.org/onto/class/google_managed_kafka_cluster"/>
    <rdfs:range rdf:resource="http://www.w3.org/2001/XMLSchema#string"/>
  </owl:DatatypeProperty>
  <owl:DatatypeProperty rdf:about="http://example.org/onto/prop/google_managed_kafka_cluster_subnet">
    <rdfs:label>subnet</rdfs:label>
    <rdfs:comment>Name of the VPC subnet from which the cluster is accessible. Both broker and bootstrap server IP addresses and DNS entries are automatically created in the subnet. There can only be one subnet per network, and the subnet must be located in the same region as the cluster. The project may differ. The name of the subnet must be in the format 'projects/PROJECT_ID/regions/REGION/subnetworks/SUBNET'.</rdfs:comment>
    <rdfs:domain rdf:resource="http://example.org/onto/class/google_managed_kafka_cluster"/>
    <rdfs:range rdf:resource="http://www.w3.org/2001/XMLSchema#string"/>
  </owl:DatatypeProperty>
  <owl:DatatypeProperty rdf:about="http://example.org/onto/prop/google_managed_kafka_cluster_mode">
    <rdfs:label>mode</rdfs:label>
    <rdfs:comment>The rebalance behavior for the cluster. When not specified, defaults to 'NO_REBALANCE'. Possible values: 'MODE_UNSPECIFIED', 'NO_REBALANCE', 'AUTO_REBALANCE_ON_SCALE_UP'.</rdfs:comment>
    <rdfs:domain rdf:resource="http://example.org/onto/class/google_managed_kafka_cluster"/>
    <rdfs:range rdf:resource="http://www.w3.org/2001/XMLSchema#string"/>
  </owl:DatatypeProperty>
  <owl:DatatypeProperty rdf:about="http://example.org/onto/prop/google_managed_kafka_cluster_create">
    <rdfs:label>create</rdfs:label>
    <rdfs:domain rdf:resource="http://example.org/onto/class/google_managed_kafka_cluster"/>
    <rdfs:range rdf:resource="http://www.w3.org/2001/XMLSchema#string"/>
  </owl:DatatypeProperty>
  <owl:DatatypeProperty rdf:about="http://example.org/onto/prop/google_managed_kafka_cluster_delete">
    <rdfs:label>delete</rdfs:label>
    <rdfs:domain rdf:resource="http://example.org/onto/class/google_managed_kafka_cluster"/>
    <rdfs:range rdf:resource="http://www.w3.org/2001/XMLSchema#string"/>
  </owl:DatatypeProperty>
  <owl:DatatypeProperty rdf:about="http://example.org/onto/prop/google_managed_kafka_cluster_update">
    <rdfs:label>update</rdfs:label>
    <rdfs:domain rdf:resource="http://example.org/onto/class/google_managed_kafka_cluster"/>
    <rdfs:range rdf:resource="http://www.w3.org/2001/XMLSchema#string"/>
  </owl:DatatypeProperty>
  <owl:DatatypeProperty rdf:about="http://example.org/onto/prop/google_managed_kafka_cluster_ssl_principal_mapping_rules">
    <rdfs:label>ssl_principal_mapping_rules</rdfs:label>
    <rdfs:comment>The rules for mapping mTLS certificate Distinguished Names (DNs) to shortened principal names for Kafka ACLs. This field corresponds exactly to the ssl.principal.mapping.rules broker config and matches the format and syntax defined in the Apache Kafka documentation. Setting or modifying this field will trigger a rolling restart of the Kafka brokers to apply the change. An empty string means that the default Kafka behavior is used. Example: 'RULE:^CN=(.?),OU=ServiceUsers.$/$1@example.com/,DEFAULT'</rdfs:comment>
    <rdfs:domain rdf:resource="http://example.org/onto/class/google_managed_kafka_cluster"/>
    <rdfs:range rdf:resource="http://www.w3.org/2001/XMLSchema#string"/>
  </owl:DatatypeProperty>
  <owl:DatatypeProperty rdf:about="http://example.org/onto/prop/google_managed_kafka_cluster_ca_pool">
    <rdfs:label>ca_pool</rdfs:label>
    <rdfs:comment>The name of the CA pool to pull CA certificates from. The CA pool does not need to be in the same project or location as the Kafka cluster. Must be in the format 'projects/PROJECT_ID/locations/LOCATION/caPools/CA_POOL_ID.</rdfs:comment>
    <rdfs:domain rdf:resource="http://example.org/onto/class/google_managed_kafka_cluster"/>
    <rdfs:range rdf:resource="http://www.w3.org/2001/XMLSchema#string"/>
  </owl:DatatypeProperty>
</rdf:RDF>
