<?xml version="1.0" encoding="UTF-8"?>
<rdf:RDF
  xmlns:rdf="http://www.w3.org/1999/02/22-rdf-syntax-ns#"
  xmlns:rdfs="http://www.w3.org/2000/01/rdf-schema#"
  xmlns:owl="http://www.w3.org/2002/07/owl#"
  xmlns:xsd="http://www.w3.org/2001/XMLSchema#"
  xml:base="http://example.org/onto/">
  <owl:Class rdf:about="http://example.org/onto/class/google_compute_router_peer">
    <rdfs:label>google_compute_router_peer</rdfs:label>
    <rdfs:comment>#
#     ***     AUTO GENERATED CODE    ***    Type: Handwritten     ***
#
# ----------------------------------------------------------------------------
#
#     This code is generated by Magic Modules using the following:
#
#     Source file: https://github.com/GoogleCloudPlatform/magic-modules/tree/main/mmv1/third_party/terraform/website/docs/r/compute_router_peer.html.markdown
#
#     DO NOT EDIT this file directly. Any changes made to this file will be
#     overwritten during the next generation cycle.
#
# ----------------------------------------------------------------------------
subcategory: "Compute Engine"
description: |-
  BGP information that must be configured into the routing stack to
  establish BGP peering.
---</rdfs:comment>
  </owl:Class>
  <owl:DatatypeProperty rdf:about="http://example.org/onto/prop/google_compute_router_peer_advertise_mode">
    <rdfs:label>advertise_mode</rdfs:label>
    <rdfs:comment>User-specified flag to indicate which mode to use for advertisement.
Valid values of this enum field are: 'DEFAULT', 'CUSTOM' Default value: "DEFAULT" Possible values: ["DEFAULT", "CUSTOM"]</rdfs:comment>
    <rdfs:domain rdf:resource="http://example.org/onto/class/google_compute_router_peer"/>
    <rdfs:range rdf:resource="http://www.w3.org/2001/XMLSchema#string"/>
  </owl:DatatypeProperty>
  <owl:DatatypeProperty rdf:about="http://example.org/onto/prop/google_compute_router_peer_advertised_groups">
    <rdfs:label>advertised_groups</rdfs:label>
    <rdfs:comment>User-specified list of prefix groups to advertise in custom
mode, which currently supports the following option:

* 'ALL_SUBNETS': Advertises all of the router's own VPC subnets.
This excludes any routes learned for subnets that use VPC Network
Peering.


Note that this field can only be populated if advertiseMode is 'CUSTOM'
and overrides the list defined for the router (in the "bgp" message).
These groups are advertised in addition to any specified prefixes.
Leave this field blank to advertise no custom groups.</rdfs:comment>
    <rdfs:domain rdf:resource="http://example.org/onto/class/google_compute_router_peer"/>
    <rdfs:range rdf:resource="http://www.w3.org/2001/XMLSchema#string"/>
  </owl:DatatypeProperty>
  <owl:DatatypeProperty rdf:about="http://example.org/onto/prop/google_compute_router_peer_advertised_route_priority">
    <rdfs:label>advertised_route_priority</rdfs:label>
    <rdfs:comment>The priority of routes advertised to this BGP peer.
Where there is more than one matching route of maximum
length, the routes with the lowest priority value win.</rdfs:comment>
    <rdfs:domain rdf:resource="http://example.org/onto/class/google_compute_router_peer"/>
    <rdfs:range rdf:resource="http://www.w3.org/2001/XMLSchema#string"/>
  </owl:DatatypeProperty>
  <owl:DatatypeProperty rdf:about="http://example.org/onto/prop/google_compute_router_peer_custom_learned_route_priority">
    <rdfs:label>custom_learned_route_priority</rdfs:label>
    <rdfs:comment>The user-defined custom learned route priority for a BGP session.
This value is applied to all custom learned route ranges for the session. You can choose a value
from 0 to 65335. If you don't provide a value, Google Cloud assigns a priority of 100 to the ranges.</rdfs:comment>
    <rdfs:domain rdf:resource="http://example.org/onto/class/google_compute_router_peer"/>
    <rdfs:range rdf:resource="http://www.w3.org/2001/XMLSchema#string"/>
  </owl:DatatypeProperty>
  <owl:DatatypeProperty rdf:about="http://example.org/onto/prop/google_compute_router_peer_enable">
    <rdfs:label>enable</rdfs:label>
    <rdfs:comment>The status of the BGP peer connection. If set to false, any active session
with the peer is terminated and all associated routing information is removed.
If set to true, the peer connection can be established with routing information.
The default is true.</rdfs:comment>
    <rdfs:domain rdf:resource="http://example.org/onto/class/google_compute_router_peer"/>
    <rdfs:range rdf:resource="http://www.w3.org/2001/XMLSchema#string"/>
  </owl:DatatypeProperty>
  <owl:DatatypeProperty rdf:about="http://example.org/onto/prop/google_compute_router_peer_enable_ipv4">
    <rdfs:label>enable_ipv4</rdfs:label>
    <rdfs:comment>Enable IPv4 traffic over BGP Peer. It is enabled by default if the peerIpAddress is version 4.</rdfs:comment>
    <rdfs:domain rdf:resource="http://example.org/onto/class/google_compute_router_peer"/>
    <rdfs:range rdf:resource="http://www.w3.org/2001/XMLSchema#string"/>
  </owl:DatatypeProperty>
  <owl:DatatypeProperty rdf:about="http://example.org/onto/prop/google_compute_router_peer_enable_ipv6">
    <rdfs:label>enable_ipv6</rdfs:label>
    <rdfs:comment>Enable IPv6 traffic over BGP Peer. If not specified, it is disabled by default.</rdfs:comment>
    <rdfs:domain rdf:resource="http://example.org/onto/class/google_compute_router_peer"/>
    <rdfs:range rdf:resource="http://www.w3.org/2001/XMLSchema#string"/>
  </owl:DatatypeProperty>
  <owl:DatatypeProperty rdf:about="http://example.org/onto/prop/google_compute_router_peer_export_policies">
    <rdfs:label>export_policies</rdfs:label>
    <rdfs:comment>routers.list of export policies applied to this peer, in the order they must be evaluated. 
The name must correspond to an existing policy that has ROUTE_POLICY_TYPE_EXPORT type.</rdfs:comment>
    <rdfs:domain rdf:resource="http://example.org/onto/class/google_compute_router_peer"/>
    <rdfs:range rdf:resource="http://www.w3.org/2001/XMLSchema#string"/>
  </owl:DatatypeProperty>
  <owl:DatatypeProperty rdf:about="http://example.org/onto/prop/google_compute_router_peer_id">
    <rdfs:label>id</rdfs:label>
    <rdfs:domain rdf:resource="http://example.org/onto/class/google_compute_router_peer"/>
    <rdfs:range rdf:resource="http://www.w3.org/2001/XMLSchema#string"/>
  </owl:DatatypeProperty>
  <owl:DatatypeProperty rdf:about="http://example.org/onto/prop/google_compute_router_peer_import_policies">
    <rdfs:label>import_policies</rdfs:label>
    <rdfs:comment>routers.list of import policies applied to this peer, in the order they must be evaluated. 
The name must correspond to an existing policy that has ROUTE_POLICY_TYPE_IMPORT type.</rdfs:comment>
    <rdfs:domain rdf:resource="http://example.org/onto/class/google_compute_router_peer"/>
    <rdfs:range rdf:resource="http://www.w3.org/2001/XMLSchema#string"/>
  </owl:DatatypeProperty>
  <owl:DatatypeProperty rdf:about="http://example.org/onto/prop/google_compute_router_peer_interface">
    <rdfs:label>interface</rdfs:label>
    <rdfs:comment>Name of the interface the BGP peer is associated with.</rdfs:comment>
    <rdfs:domain rdf:resource="http://example.org/onto/class/google_compute_router_peer"/>
    <rdfs:range rdf:resource="http://www.w3.org/2001/XMLSchema#string"/>
  </owl:DatatypeProperty>
  <owl:DatatypeProperty rdf:about="http://example.org/onto/prop/google_compute_router_peer_ip_address">
    <rdfs:label>ip_address</rdfs:label>
    <rdfs:comment>IP address of the interface inside Google Cloud Platform.
Only IPv4 is supported.</rdfs:comment>
    <rdfs:domain rdf:resource="http://example.org/onto/class/google_compute_router_peer"/>
    <rdfs:range rdf:resource="http://www.w3.org/2001/XMLSchema#string"/>
  </owl:DatatypeProperty>
  <owl:DatatypeProperty rdf:about="http://example.org/onto/prop/google_compute_router_peer_ipv4_nexthop_address">
    <rdfs:label>ipv4_nexthop_address</rdfs:label>
    <rdfs:comment>IPv4 address of the interface inside Google Cloud Platform.</rdfs:comment>
    <rdfs:domain rdf:resource="http://example.org/onto/class/google_compute_router_peer"/>
    <rdfs:range rdf:resource="http://www.w3.org/2001/XMLSchema#string"/>
  </owl:DatatypeProperty>
  <owl:DatatypeProperty rdf:about="http://example.org/onto/prop/google_compute_router_peer_ipv6_nexthop_address">
    <rdfs:label>ipv6_nexthop_address</rdfs:label>
    <rdfs:comment>IPv6 address of the interface inside Google Cloud Platform.
The address must be in the range 2600:2d00:0:2::/64 or 2600:2d00:0:3::/64.
If you do not specify the next hop addresses, Google Cloud automatically
assigns unused addresses from the 2600:2d00:0:2::/64 or 2600:2d00:0:3::/64 range for you.</rdfs:comment>
    <rdfs:domain rdf:resource="http://example.org/onto/class/google_compute_router_peer"/>
    <rdfs:range rdf:resource="http://www.w3.org/2001/XMLSchema#string"/>
  </owl:DatatypeProperty>
  <owl:DatatypeProperty rdf:about="http://example.org/onto/prop/google_compute_router_peer_is_advertised_route_priority_set">
    <rdfs:label>is_advertised_route_priority_set</rdfs:label>
    <rdfs:comment>An internal boolean field for provider use for zero_advertised_route_priority.</rdfs:comment>
    <rdfs:domain rdf:resource="http://example.org/onto/class/google_compute_router_peer"/>
    <rdfs:range rdf:resource="http://www.w3.org/2001/XMLSchema#string"/>
  </owl:DatatypeProperty>
  <owl:DatatypeProperty rdf:about="http://example.org/onto/prop/google_compute_router_peer_is_custom_learned_priority_set">
    <rdfs:label>is_custom_learned_priority_set</rdfs:label>
    <rdfs:comment>An internal boolean field for provider use.</rdfs:comment>
    <rdfs:domain rdf:resource="http://example.org/onto/class/google_compute_router_peer"/>
    <rdfs:range rdf:resource="http://www.w3.org/2001/XMLSchema#string"/>
  </owl:DatatypeProperty>
  <owl:DatatypeProperty rdf:about="http://example.org/onto/prop/google_compute_router_peer_management_type">
    <rdfs:label>management_type</rdfs:label>
    <rdfs:comment>The resource that configures and manages this BGP peer.

* 'MANAGED_BY_USER' is the default value and can be managed by
you or other users
* 'MANAGED_BY_ATTACHMENT' is a BGP peer that is configured and
managed by Cloud Interconnect, specifically by an
InterconnectAttachment of type PARTNER. Google automatically
creates, updates, and deletes this type of BGP peer when the
PARTNER InterconnectAttachment is created, updated,
or deleted.</rdfs:comment>
    <rdfs:domain rdf:resource="http://example.org/onto/class/google_compute_router_peer"/>
    <rdfs:range rdf:resource="http://www.w3.org/2001/XMLSchema#string"/>
  </owl:DatatypeProperty>
  <owl:DatatypeProperty rdf:about="http://example.org/onto/prop/google_compute_router_peer_name">
    <rdfs:label>name</rdfs:label>
    <rdfs:comment>Name of this BGP peer. The name must be 1-63 characters long,
and comply with RFC1035. Specifically, the name must be 1-63 characters
long and match the regular expression '[a-z]([-a-z0-9]*[a-z0-9])?' which
means the first character must be a lowercase letter, and all
following characters must be a dash, lowercase letter, or digit,
except the last character, which cannot be a dash.</rdfs:comment>
    <rdfs:domain rdf:resource="http://example.org/onto/class/google_compute_router_peer"/>
    <rdfs:range rdf:resource="http://www.w3.org/2001/XMLSchema#string"/>
  </owl:DatatypeProperty>
  <owl:DatatypeProperty rdf:about="http://example.org/onto/prop/google_compute_router_peer_peer_asn">
    <rdfs:label>peer_asn</rdfs:label>
    <rdfs:comment>Peer BGP Autonomous System Number (ASN).
Each BGP interface may use a different value.</rdfs:comment>
    <rdfs:domain rdf:resource="http://example.org/onto/class/google_compute_router_peer"/>
    <rdfs:range rdf:resource="http://www.w3.org/2001/XMLSchema#string"/>
  </owl:DatatypeProperty>
  <owl:DatatypeProperty rdf:about="http://example.org/onto/prop/google_compute_router_peer_peer_ip_address">
    <rdfs:label>peer_ip_address</rdfs:label>
    <rdfs:comment>IP address of the BGP interface outside Google Cloud Platform.
Only IPv4 is supported. Required if 'ip_address' is set.</rdfs:comment>
    <rdfs:domain rdf:resource="http://example.org/onto/class/google_compute_router_peer"/>
    <rdfs:range rdf:resource="http://www.w3.org/2001/XMLSchema#string"/>
  </owl:DatatypeProperty>
  <owl:DatatypeProperty rdf:about="http://example.org/onto/prop/google_compute_router_peer_peer_ipv4_nexthop_address">
    <rdfs:label>peer_ipv4_nexthop_address</rdfs:label>
    <rdfs:comment>IPv4 address of the BGP interface outside Google Cloud Platform.</rdfs:comment>
    <rdfs:domain rdf:resource="http://example.org/onto/class/google_compute_router_peer"/>
    <rdfs:range rdf:resource="http://www.w3.org/2001/XMLSchema#string"/>
  </owl:DatatypeProperty>
  <owl:DatatypeProperty rdf:about="http://example.org/onto/prop/google_compute_router_peer_peer_ipv6_nexthop_address">
    <rdfs:label>peer_ipv6_nexthop_address</rdfs:label>
    <rdfs:comment>IPv6 address of the BGP interface outside Google Cloud Platform.
The address must be in the range 2600:2d00:0:2::/64 or 2600:2d00:0:3::/64.
If you do not specify the next hop addresses, Google Cloud automatically
assigns unused addresses from the 2600:2d00:0:2::/64 or 2600:2d00:0:3::/64 range for you.</rdfs:comment>
    <rdfs:domain rdf:resource="http://example.org/onto/class/google_compute_router_peer"/>
    <rdfs:range rdf:resource="http://www.w3.org/2001/XMLSchema#string"/>
  </owl:DatatypeProperty>
  <owl:DatatypeProperty rdf:about="http://example.org/onto/prop/google_compute_router_peer_project">
    <rdfs:label>project</rdfs:label>
    <rdfs:domain rdf:resource="http://example.org/onto/class/google_compute_router_peer"/>
    <rdfs:range rdf:resource="http://www.w3.org/2001/XMLSchema#string"/>
  </owl:DatatypeProperty>
  <owl:DatatypeProperty rdf:about="http://example.org/onto/prop/google_compute_router_peer_region">
    <rdfs:label>region</rdfs:label>
    <rdfs:comment>Region where the router and BgpPeer reside.
If it is not provided, the provider region is used.</rdfs:comment>
    <rdfs:domain rdf:resource="http://example.org/onto/class/google_compute_router_peer"/>
    <rdfs:range rdf:resource="http://www.w3.org/2001/XMLSchema#string"/>
  </owl:DatatypeProperty>
  <owl:DatatypeProperty rdf:about="http://example.org/onto/prop/google_compute_router_peer_router">
    <rdfs:label>router</rdfs:label>
    <rdfs:comment>The name of the Cloud Router in which this BgpPeer will be configured.</rdfs:comment>
    <rdfs:domain rdf:resource="http://example.org/onto/class/google_compute_router_peer"/>
    <rdfs:range rdf:resource="http://www.w3.org/2001/XMLSchema#string"/>
  </owl:DatatypeProperty>
  <owl:DatatypeProperty rdf:about="http://example.org/onto/prop/google_compute_router_peer_router_appliance_instance">
    <rdfs:label>router_appliance_instance</rdfs:label>
    <rdfs:comment>The URI of the VM instance that is used as third-party router appliances
such as Next Gen Firewalls, Virtual Routers, or Router Appliances.
The VM instance must be located in zones contained in the same region as
this Cloud Router. The VM instance is the peer side of the BGP session.</rdfs:comment>
    <rdfs:domain rdf:resource="http://example.org/onto/class/google_compute_router_peer"/>
    <rdfs:range rdf:resource="http://www.w3.org/2001/XMLSchema#string"/>
  </owl:DatatypeProperty>
  <owl:DatatypeProperty rdf:about="http://example.org/onto/prop/google_compute_router_peer_zero_advertised_route_priority">
    <rdfs:label>zero_advertised_route_priority</rdfs:label>
    <rdfs:comment>Force the advertised_route_priority to be 0.</rdfs:comment>
    <rdfs:domain rdf:resource="http://example.org/onto/class/google_compute_router_peer"/>
    <rdfs:range rdf:resource="http://www.w3.org/2001/XMLSchema#string"/>
  </owl:DatatypeProperty>
  <owl:DatatypeProperty rdf:about="http://example.org/onto/prop/google_compute_router_peer_zero_custom_learned_route_priority">
    <rdfs:label>zero_custom_learned_route_priority</rdfs:label>
    <rdfs:comment>Force the custom_learned_route_priority to be 0.</rdfs:comment>
    <rdfs:domain rdf:resource="http://example.org/onto/class/google_compute_router_peer"/>
    <rdfs:range rdf:resource="http://www.w3.org/2001/XMLSchema#string"/>
  </owl:DatatypeProperty>
  <owl:DatatypeProperty rdf:about="http://example.org/onto/prop/google_compute_router_peer_description">
    <rdfs:label>description</rdfs:label>
    <rdfs:comment>User-specified description for the IP range.</rdfs:comment>
    <rdfs:domain rdf:resource="http://example.org/onto/class/google_compute_router_peer"/>
    <rdfs:range rdf:resource="http://www.w3.org/2001/XMLSchema#string"/>
  </owl:DatatypeProperty>
  <owl:DatatypeProperty rdf:about="http://example.org/onto/prop/google_compute_router_peer_range">
    <rdfs:label>range</rdfs:label>
    <rdfs:comment>The IP range to advertise. The value must be a
CIDR-formatted string.</rdfs:comment>
    <rdfs:domain rdf:resource="http://example.org/onto/class/google_compute_router_peer"/>
    <rdfs:range rdf:resource="http://www.w3.org/2001/XMLSchema#string"/>
  </owl:DatatypeProperty>
  <owl:DatatypeProperty rdf:about="http://example.org/onto/prop/google_compute_router_peer_min_receive_interval">
    <rdfs:label>min_receive_interval</rdfs:label>
    <rdfs:comment>The minimum interval, in milliseconds, between BFD control packets
received from the peer router. The actual value is negotiated
between the two routers and is equal to the greater of this value
and the transmit interval of the other router. If set, this value
must be between 1000 and 30000.</rdfs:comment>
    <rdfs:domain rdf:resource="http://example.org/onto/class/google_compute_router_peer"/>
    <rdfs:range rdf:resource="http://www.w3.org/2001/XMLSchema#string"/>
  </owl:DatatypeProperty>
  <owl:DatatypeProperty rdf:about="http://example.org/onto/prop/google_compute_router_peer_min_transmit_interval">
    <rdfs:label>min_transmit_interval</rdfs:label>
    <rdfs:comment>The minimum interval, in milliseconds, between BFD control packets
transmitted to the peer router. The actual value is negotiated
between the two routers and is equal to the greater of this value
and the corresponding receive interval of the other router. If set,
this value must be between 1000 and 30000.</rdfs:comment>
    <rdfs:domain rdf:resource="http://example.org/onto/class/google_compute_router_peer"/>
    <rdfs:range rdf:resource="http://www.w3.org/2001/XMLSchema#string"/>
  </owl:DatatypeProperty>
  <owl:DatatypeProperty rdf:about="http://example.org/onto/prop/google_compute_router_peer_multiplier">
    <rdfs:label>multiplier</rdfs:label>
    <rdfs:comment>The number of consecutive BFD packets that must be missed before
BFD declares that a peer is unavailable. If set, the value must
be a value between 5 and 16.</rdfs:comment>
    <rdfs:domain rdf:resource="http://example.org/onto/class/google_compute_router_peer"/>
    <rdfs:range rdf:resource="http://www.w3.org/2001/XMLSchema#string"/>
  </owl:DatatypeProperty>
  <owl:DatatypeProperty rdf:about="http://example.org/onto/prop/google_compute_router_peer_session_initialization_mode">
    <rdfs:label>session_initialization_mode</rdfs:label>
    <rdfs:comment>The BFD session initialization mode for this BGP peer.
If set to 'ACTIVE', the Cloud Router will initiate the BFD session
for this BGP peer. If set to 'PASSIVE', the Cloud Router will wait
for the peer router to initiate the BFD session for this BGP peer.
If set to 'DISABLED', BFD is disabled for this BGP peer. Possible values: ["ACTIVE", "DISABLED", "PASSIVE"]</rdfs:comment>
    <rdfs:domain rdf:resource="http://example.org/onto/class/google_compute_router_peer"/>
    <rdfs:range rdf:resource="http://www.w3.org/2001/XMLSchema#string"/>
  </owl:DatatypeProperty>
  <owl:DatatypeProperty rdf:about="http://example.org/onto/prop/google_compute_router_peer_range">
    <rdfs:label>range</rdfs:label>
    <rdfs:comment>The IP range to learn. The value must be a
CIDR-formatted string.</rdfs:comment>
    <rdfs:domain rdf:resource="http://example.org/onto/class/google_compute_router_peer"/>
    <rdfs:range rdf:resource="http://www.w3.org/2001/XMLSchema#string"/>
  </owl:DatatypeProperty>
  <owl:DatatypeProperty rdf:about="http://example.org/onto/prop/google_compute_router_peer_key">
    <rdfs:label>key</rdfs:label>
    <rdfs:comment>Value of the key.</rdfs:comment>
    <rdfs:domain rdf:resource="http://example.org/onto/class/google_compute_router_peer"/>
    <rdfs:range rdf:resource="http://www.w3.org/2001/XMLSchema#string"/>
  </owl:DatatypeProperty>
  <owl:DatatypeProperty rdf:about="http://example.org/onto/prop/google_compute_router_peer_name">
    <rdfs:label>name</rdfs:label>
    <rdfs:comment>[REQUIRED] Name used to identify the key.
Must be unique within a router. Must be referenced by exactly one bgpPeer. Must comply with RFC1035.</rdfs:comment>
    <rdfs:domain rdf:resource="http://example.org/onto/class/google_compute_router_peer"/>
    <rdfs:range rdf:resource="http://www.w3.org/2001/XMLSchema#string"/>
  </owl:DatatypeProperty>
  <owl:DatatypeProperty rdf:about="http://example.org/onto/prop/google_compute_router_peer_create">
    <rdfs:label>create</rdfs:label>
    <rdfs:domain rdf:resource="http://example.org/onto/class/google_compute_router_peer"/>
    <rdfs:range rdf:resource="http://www.w3.org/2001/XMLSchema#string"/>
  </owl:DatatypeProperty>
  <owl:DatatypeProperty rdf:about="http://example.org/onto/prop/google_compute_router_peer_delete">
    <rdfs:label>delete</rdfs:label>
    <rdfs:domain rdf:resource="http://example.org/onto/class/google_compute_router_peer"/>
    <rdfs:range rdf:resource="http://www.w3.org/2001/XMLSchema#string"/>
  </owl:DatatypeProperty>
  <owl:DatatypeProperty rdf:about="http://example.org/onto/prop/google_compute_router_peer_update">
    <rdfs:label>update</rdfs:label>
    <rdfs:domain rdf:resource="http://example.org/onto/class/google_compute_router_peer"/>
    <rdfs:range rdf:resource="http://www.w3.org/2001/XMLSchema#string"/>
  </owl:DatatypeProperty>
</rdf:RDF>
