<?xml version="1.0" encoding="UTF-8"?>
<rdf:RDF
  xmlns:rdf="http://www.w3.org/1999/02/22-rdf-syntax-ns#"
  xmlns:rdfs="http://www.w3.org/2000/01/rdf-schema#"
  xmlns:owl="http://www.w3.org/2002/07/owl#"
  xmlns:xsd="http://www.w3.org/2001/XMLSchema#"
  xml:base="http://example.org/onto/">
  <owl:Class rdf:about="http://example.org/onto/class/google_dataproc_session_template">
    <rdfs:label>google_dataproc_session_template</rdfs:label>
    <rdfs:comment>#
#     ***     AUTO GENERATED CODE    ***    Type: MMv1     ***
#
# ----------------------------------------------------------------------------
#
#     This code is generated by Magic Modules using the following:
#
#     Configuration: https:#github.com/GoogleCloudPlatform/magic-modules/tree/main/mmv1/products/dataproc/SessionTemplate.yaml
#     Template:      https:#github.com/GoogleCloudPlatform/magic-modules/tree/main/mmv1/templates/terraform/resource.html.markdown.tmpl
#
#     DO NOT EDIT this file directly. Any changes made to this file will be
#     overwritten during the next generation cycle.
#
# ----------------------------------------------------------------------------
subcategory: "Dataproc"
description: |-
  A Dataproc Serverless session template defines the configuration settings for
  creating one or more Dataproc Serverless interactive sessions.
---</rdfs:comment>
  </owl:Class>
  <owl:DatatypeProperty rdf:about="http://example.org/onto/prop/google_dataproc_session_template_create_time">
    <rdfs:label>create_time</rdfs:label>
    <rdfs:comment>The time when the session template was created.</rdfs:comment>
    <rdfs:domain rdf:resource="http://example.org/onto/class/google_dataproc_session_template"/>
    <rdfs:range rdf:resource="http://www.w3.org/2001/XMLSchema#string"/>
  </owl:DatatypeProperty>
  <owl:DatatypeProperty rdf:about="http://example.org/onto/prop/google_dataproc_session_template_creator">
    <rdfs:label>creator</rdfs:label>
    <rdfs:comment>The email address of the user who created the session template.</rdfs:comment>
    <rdfs:domain rdf:resource="http://example.org/onto/class/google_dataproc_session_template"/>
    <rdfs:range rdf:resource="http://www.w3.org/2001/XMLSchema#string"/>
  </owl:DatatypeProperty>
  <owl:DatatypeProperty rdf:about="http://example.org/onto/prop/google_dataproc_session_template_effective_labels">
    <rdfs:label>effective_labels</rdfs:label>
    <rdfs:comment>All of labels (key/value pairs) present on the resource in GCP, including the labels configured through Terraform, other clients and services.</rdfs:comment>
    <rdfs:domain rdf:resource="http://example.org/onto/class/google_dataproc_session_template"/>
    <rdfs:range rdf:resource="http://www.w3.org/2001/XMLSchema#string"/>
  </owl:DatatypeProperty>
  <owl:DatatypeProperty rdf:about="http://example.org/onto/prop/google_dataproc_session_template_id">
    <rdfs:label>id</rdfs:label>
    <rdfs:domain rdf:resource="http://example.org/onto/class/google_dataproc_session_template"/>
    <rdfs:range rdf:resource="http://www.w3.org/2001/XMLSchema#string"/>
  </owl:DatatypeProperty>
  <owl:DatatypeProperty rdf:about="http://example.org/onto/prop/google_dataproc_session_template_labels">
    <rdfs:label>labels</rdfs:label>
    <rdfs:comment>The labels to associate with this session template.


**Note**: This field is non-authoritative, and will only manage the labels present in your configuration.
Please refer to the field 'effective_labels' for all of the labels present on the resource.</rdfs:comment>
    <rdfs:domain rdf:resource="http://example.org/onto/class/google_dataproc_session_template"/>
    <rdfs:range rdf:resource="http://www.w3.org/2001/XMLSchema#string"/>
  </owl:DatatypeProperty>
  <owl:DatatypeProperty rdf:about="http://example.org/onto/prop/google_dataproc_session_template_location">
    <rdfs:label>location</rdfs:label>
    <rdfs:comment>The location in which the session template will be created in.</rdfs:comment>
    <rdfs:domain rdf:resource="http://example.org/onto/class/google_dataproc_session_template"/>
    <rdfs:range rdf:resource="http://www.w3.org/2001/XMLSchema#string"/>
  </owl:DatatypeProperty>
  <owl:DatatypeProperty rdf:about="http://example.org/onto/prop/google_dataproc_session_template_name">
    <rdfs:label>name</rdfs:label>
    <rdfs:comment>The resource name of the session template in the following format:
projects/{project}/locations/{location}/sessionTemplates/{template_id}</rdfs:comment>
    <rdfs:domain rdf:resource="http://example.org/onto/class/google_dataproc_session_template"/>
    <rdfs:range rdf:resource="http://www.w3.org/2001/XMLSchema#string"/>
  </owl:DatatypeProperty>
  <owl:DatatypeProperty rdf:about="http://example.org/onto/prop/google_dataproc_session_template_project">
    <rdfs:label>project</rdfs:label>
    <rdfs:domain rdf:resource="http://example.org/onto/class/google_dataproc_session_template"/>
    <rdfs:range rdf:resource="http://www.w3.org/2001/XMLSchema#string"/>
  </owl:DatatypeProperty>
  <owl:DatatypeProperty rdf:about="http://example.org/onto/prop/google_dataproc_session_template_terraform_labels">
    <rdfs:label>terraform_labels</rdfs:label>
    <rdfs:comment>The combination of labels configured directly on the resource
 and default labels configured on the provider.</rdfs:comment>
    <rdfs:domain rdf:resource="http://example.org/onto/class/google_dataproc_session_template"/>
    <rdfs:range rdf:resource="http://www.w3.org/2001/XMLSchema#string"/>
  </owl:DatatypeProperty>
  <owl:DatatypeProperty rdf:about="http://example.org/onto/prop/google_dataproc_session_template_update_time">
    <rdfs:label>update_time</rdfs:label>
    <rdfs:comment>The time when the session template was updated.</rdfs:comment>
    <rdfs:domain rdf:resource="http://example.org/onto/class/google_dataproc_session_template"/>
    <rdfs:range rdf:resource="http://www.w3.org/2001/XMLSchema#string"/>
  </owl:DatatypeProperty>
  <owl:DatatypeProperty rdf:about="http://example.org/onto/prop/google_dataproc_session_template_uuid">
    <rdfs:label>uuid</rdfs:label>
    <rdfs:comment>A session template UUID (Unique Universal Identifier). The service generates this value when it creates the session template.</rdfs:comment>
    <rdfs:domain rdf:resource="http://example.org/onto/class/google_dataproc_session_template"/>
    <rdfs:range rdf:resource="http://www.w3.org/2001/XMLSchema#string"/>
  </owl:DatatypeProperty>
  <owl:DatatypeProperty rdf:about="http://example.org/onto/prop/google_dataproc_session_template_idle_ttl">
    <rdfs:label>idle_ttl</rdfs:label>
    <rdfs:comment>The duration to keep the session alive while it's idling.
Exceeding this threshold causes the session to terminate. Minimum value is 10 minutes; maximum value is 14 day.
Defaults to 1 hour if not set. If both ttl and idleTtl are specified for an interactive session, the conditions
are treated as OR conditions: the workload will be terminated when it has been idle for idleTtl or when ttl has
been exceeded, whichever occurs first.</rdfs:comment>
    <rdfs:domain rdf:resource="http://example.org/onto/class/google_dataproc_session_template"/>
    <rdfs:range rdf:resource="http://www.w3.org/2001/XMLSchema#string"/>
  </owl:DatatypeProperty>
  <owl:DatatypeProperty rdf:about="http://example.org/onto/prop/google_dataproc_session_template_kms_key">
    <rdfs:label>kms_key</rdfs:label>
    <rdfs:comment>The Cloud KMS key to use for encryption.</rdfs:comment>
    <rdfs:domain rdf:resource="http://example.org/onto/class/google_dataproc_session_template"/>
    <rdfs:range rdf:resource="http://www.w3.org/2001/XMLSchema#string"/>
  </owl:DatatypeProperty>
  <owl:DatatypeProperty rdf:about="http://example.org/onto/prop/google_dataproc_session_template_network_tags">
    <rdfs:label>network_tags</rdfs:label>
    <rdfs:comment>Tags used for network traffic control.</rdfs:comment>
    <rdfs:domain rdf:resource="http://example.org/onto/class/google_dataproc_session_template"/>
    <rdfs:range rdf:resource="http://www.w3.org/2001/XMLSchema#string"/>
  </owl:DatatypeProperty>
  <owl:DatatypeProperty rdf:about="http://example.org/onto/prop/google_dataproc_session_template_service_account">
    <rdfs:label>service_account</rdfs:label>
    <rdfs:comment>Service account that used to execute workload.</rdfs:comment>
    <rdfs:domain rdf:resource="http://example.org/onto/class/google_dataproc_session_template"/>
    <rdfs:range rdf:resource="http://www.w3.org/2001/XMLSchema#string"/>
  </owl:DatatypeProperty>
  <owl:DatatypeProperty rdf:about="http://example.org/onto/prop/google_dataproc_session_template_staging_bucket">
    <rdfs:label>staging_bucket</rdfs:label>
    <rdfs:comment>A Cloud Storage bucket used to stage workload dependencies, config files, and store
workload output and other ephemeral data, such as Spark history files. If you do not specify a staging bucket,
Cloud Dataproc will determine a Cloud Storage location according to the region where your workload is running,
and then create and manage project-level, per-location staging and temporary buckets.
This field requires a Cloud Storage bucket name, not a gs://... URI to a Cloud Storage bucket.</rdfs:comment>
    <rdfs:domain rdf:resource="http://example.org/onto/class/google_dataproc_session_template"/>
    <rdfs:range rdf:resource="http://www.w3.org/2001/XMLSchema#string"/>
  </owl:DatatypeProperty>
  <owl:DatatypeProperty rdf:about="http://example.org/onto/prop/google_dataproc_session_template_subnetwork_uri">
    <rdfs:label>subnetwork_uri</rdfs:label>
    <rdfs:comment>Subnetwork configuration for workload execution.</rdfs:comment>
    <rdfs:domain rdf:resource="http://example.org/onto/class/google_dataproc_session_template"/>
    <rdfs:range rdf:resource="http://www.w3.org/2001/XMLSchema#string"/>
  </owl:DatatypeProperty>
  <owl:DatatypeProperty rdf:about="http://example.org/onto/prop/google_dataproc_session_template_ttl">
    <rdfs:label>ttl</rdfs:label>
    <rdfs:comment>The duration after which the workload will be terminated.
When the workload exceeds this duration, it will be unconditionally terminated without waiting for ongoing
work to finish. If ttl is not specified for a session workload, the workload will be allowed to run until it
exits naturally (or run forever without exiting). If ttl is not specified for an interactive session,
it defaults to 24 hours. If ttl is not specified for a batch that uses 2.1+ runtime version, it defaults to 4 hours.
Minimum value is 10 minutes; maximum value is 14 days. If both ttl and idleTtl are specified (for an interactive session),
the conditions are treated as OR conditions: the workload will be terminated when it has been idle for idleTtl or
when ttl has been exceeded, whichever occurs first.</rdfs:comment>
    <rdfs:domain rdf:resource="http://example.org/onto/class/google_dataproc_session_template"/>
    <rdfs:range rdf:resource="http://www.w3.org/2001/XMLSchema#string"/>
  </owl:DatatypeProperty>
  <owl:DatatypeProperty rdf:about="http://example.org/onto/prop/google_dataproc_session_template_user_workload_authentication_type">
    <rdfs:label>user_workload_authentication_type</rdfs:label>
    <rdfs:comment>Authentication type for the user workload running in containers. Possible values: ["SERVICE_ACCOUNT", "END_USER_CREDENTIALS"]</rdfs:comment>
    <rdfs:domain rdf:resource="http://example.org/onto/class/google_dataproc_session_template"/>
    <rdfs:range rdf:resource="http://www.w3.org/2001/XMLSchema#string"/>
  </owl:DatatypeProperty>
  <owl:DatatypeProperty rdf:about="http://example.org/onto/prop/google_dataproc_session_template_metastore_service">
    <rdfs:label>metastore_service</rdfs:label>
    <rdfs:comment>Resource name of an existing Dataproc Metastore service.</rdfs:comment>
    <rdfs:domain rdf:resource="http://example.org/onto/class/google_dataproc_session_template"/>
    <rdfs:range rdf:resource="http://www.w3.org/2001/XMLSchema#string"/>
  </owl:DatatypeProperty>
  <owl:DatatypeProperty rdf:about="http://example.org/onto/prop/google_dataproc_session_template_dataproc_cluster">
    <rdfs:label>dataproc_cluster</rdfs:label>
    <rdfs:comment>Resource name of an existing Dataproc Cluster to act as a Spark History Server for the workload.</rdfs:comment>
    <rdfs:domain rdf:resource="http://example.org/onto/class/google_dataproc_session_template"/>
    <rdfs:range rdf:resource="http://www.w3.org/2001/XMLSchema#string"/>
  </owl:DatatypeProperty>
  <owl:DatatypeProperty rdf:about="http://example.org/onto/prop/google_dataproc_session_template_display_name">
    <rdfs:label>display_name</rdfs:label>
    <rdfs:comment>Display name, shown in the Jupyter kernelspec card.</rdfs:comment>
    <rdfs:domain rdf:resource="http://example.org/onto/class/google_dataproc_session_template"/>
    <rdfs:range rdf:resource="http://www.w3.org/2001/XMLSchema#string"/>
  </owl:DatatypeProperty>
  <owl:DatatypeProperty rdf:about="http://example.org/onto/prop/google_dataproc_session_template_kernel">
    <rdfs:label>kernel</rdfs:label>
    <rdfs:comment>Kernel to be used with Jupyter interactive session. Possible values: ["PYTHON", "SCALA"]</rdfs:comment>
    <rdfs:domain rdf:resource="http://example.org/onto/class/google_dataproc_session_template"/>
    <rdfs:range rdf:resource="http://www.w3.org/2001/XMLSchema#string"/>
  </owl:DatatypeProperty>
  <owl:DatatypeProperty rdf:about="http://example.org/onto/prop/google_dataproc_session_template_container_image">
    <rdfs:label>container_image</rdfs:label>
    <rdfs:comment>Optional custom container image for the job runtime environment. If not specified, a default container image will be used.</rdfs:comment>
    <rdfs:domain rdf:resource="http://example.org/onto/class/google_dataproc_session_template"/>
    <rdfs:range rdf:resource="http://www.w3.org/2001/XMLSchema#string"/>
  </owl:DatatypeProperty>
  <owl:DatatypeProperty rdf:about="http://example.org/onto/prop/google_dataproc_session_template_effective_properties">
    <rdfs:label>effective_properties</rdfs:label>
    <rdfs:comment>A mapping of property names to values, which are used to configure workload execution.</rdfs:comment>
    <rdfs:domain rdf:resource="http://example.org/onto/class/google_dataproc_session_template"/>
    <rdfs:range rdf:resource="http://www.w3.org/2001/XMLSchema#string"/>
  </owl:DatatypeProperty>
  <owl:DatatypeProperty rdf:about="http://example.org/onto/prop/google_dataproc_session_template_properties">
    <rdfs:label>properties</rdfs:label>
    <rdfs:comment>A mapping of property names to values, which are used to configure workload execution.</rdfs:comment>
    <rdfs:domain rdf:resource="http://example.org/onto/class/google_dataproc_session_template"/>
    <rdfs:range rdf:resource="http://www.w3.org/2001/XMLSchema#string"/>
  </owl:DatatypeProperty>
  <owl:DatatypeProperty rdf:about="http://example.org/onto/prop/google_dataproc_session_template_version">
    <rdfs:label>version</rdfs:label>
    <rdfs:comment>Version of the session runtime.</rdfs:comment>
    <rdfs:domain rdf:resource="http://example.org/onto/class/google_dataproc_session_template"/>
    <rdfs:range rdf:resource="http://www.w3.org/2001/XMLSchema#string"/>
  </owl:DatatypeProperty>
  <owl:DatatypeProperty rdf:about="http://example.org/onto/prop/google_dataproc_session_template_create">
    <rdfs:label>create</rdfs:label>
    <rdfs:domain rdf:resource="http://example.org/onto/class/google_dataproc_session_template"/>
    <rdfs:range rdf:resource="http://www.w3.org/2001/XMLSchema#string"/>
  </owl:DatatypeProperty>
  <owl:DatatypeProperty rdf:about="http://example.org/onto/prop/google_dataproc_session_template_delete">
    <rdfs:label>delete</rdfs:label>
    <rdfs:domain rdf:resource="http://example.org/onto/class/google_dataproc_session_template"/>
    <rdfs:range rdf:resource="http://www.w3.org/2001/XMLSchema#string"/>
  </owl:DatatypeProperty>
  <owl:DatatypeProperty rdf:about="http://example.org/onto/prop/google_dataproc_session_template_update">
    <rdfs:label>update</rdfs:label>
    <rdfs:domain rdf:resource="http://example.org/onto/class/google_dataproc_session_template"/>
    <rdfs:range rdf:resource="http://www.w3.org/2001/XMLSchema#string"/>
  </owl:DatatypeProperty>
</rdf:RDF>
