<?xml version="1.0" encoding="UTF-8"?>
<rdf:RDF
  xmlns:rdf="http://www.w3.org/1999/02/22-rdf-syntax-ns#"
  xmlns:rdfs="http://www.w3.org/2000/01/rdf-schema#"
  xmlns:owl="http://www.w3.org/2002/07/owl#"
  xmlns:xsd="http://www.w3.org/2001/XMLSchema#"
  xml:base="http://example.org/onto/">
  <owl:Class rdf:about="http://example.org/onto/class/google_cloudbuild_bitbucket_server_config">
    <rdfs:label>google_cloudbuild_bitbucket_server_config</rdfs:label>
    <rdfs:comment>#
#     ***     AUTO GENERATED CODE    ***    Type: MMv1     ***
#
# ----------------------------------------------------------------------------
#
#     This code is generated by Magic Modules using the following:
#
#     Configuration: https:#github.com/GoogleCloudPlatform/magic-modules/tree/main/mmv1/products/cloudbuild/BitbucketServerConfig.yaml
#     Template:      https:#github.com/GoogleCloudPlatform/magic-modules/tree/main/mmv1/templates/terraform/resource.html.markdown.tmpl
#
#     DO NOT EDIT this file directly. Any changes made to this file will be
#     overwritten during the next generation cycle.
#
# ----------------------------------------------------------------------------
subcategory: "Cloud Build"
description: |-
  BitbucketServerConfig represents the configuration for a Bitbucket Server.
---</rdfs:comment>
  </owl:Class>
  <owl:DatatypeProperty rdf:about="http://example.org/onto/prop/google_cloudbuild_bitbucket_server_config_api_key">
    <rdfs:label>api_key</rdfs:label>
    <rdfs:comment>Immutable. API Key that will be attached to webhook. Once this field has been set, it cannot be changed.
Changing this field will result in deleting/ recreating the resource.</rdfs:comment>
    <rdfs:domain rdf:resource="http://example.org/onto/class/google_cloudbuild_bitbucket_server_config"/>
    <rdfs:range rdf:resource="http://www.w3.org/2001/XMLSchema#string"/>
  </owl:DatatypeProperty>
  <owl:DatatypeProperty rdf:about="http://example.org/onto/prop/google_cloudbuild_bitbucket_server_config_config_id">
    <rdfs:label>config_id</rdfs:label>
    <rdfs:comment>The ID to use for the BitbucketServerConfig, which will become the final component of the BitbucketServerConfig's resource name.</rdfs:comment>
    <rdfs:domain rdf:resource="http://example.org/onto/class/google_cloudbuild_bitbucket_server_config"/>
    <rdfs:range rdf:resource="http://www.w3.org/2001/XMLSchema#string"/>
  </owl:DatatypeProperty>
  <owl:DatatypeProperty rdf:about="http://example.org/onto/prop/google_cloudbuild_bitbucket_server_config_host_uri">
    <rdfs:label>host_uri</rdfs:label>
    <rdfs:comment>Immutable. The URI of the Bitbucket Server host. Once this field has been set, it cannot be changed.
If you need to change it, please create another BitbucketServerConfig.</rdfs:comment>
    <rdfs:domain rdf:resource="http://example.org/onto/class/google_cloudbuild_bitbucket_server_config"/>
    <rdfs:range rdf:resource="http://www.w3.org/2001/XMLSchema#string"/>
  </owl:DatatypeProperty>
  <owl:DatatypeProperty rdf:about="http://example.org/onto/prop/google_cloudbuild_bitbucket_server_config_id">
    <rdfs:label>id</rdfs:label>
    <rdfs:domain rdf:resource="http://example.org/onto/class/google_cloudbuild_bitbucket_server_config"/>
    <rdfs:range rdf:resource="http://www.w3.org/2001/XMLSchema#string"/>
  </owl:DatatypeProperty>
  <owl:DatatypeProperty rdf:about="http://example.org/onto/prop/google_cloudbuild_bitbucket_server_config_location">
    <rdfs:label>location</rdfs:label>
    <rdfs:comment>The location of this bitbucket server config.</rdfs:comment>
    <rdfs:domain rdf:resource="http://example.org/onto/class/google_cloudbuild_bitbucket_server_config"/>
    <rdfs:range rdf:resource="http://www.w3.org/2001/XMLSchema#string"/>
  </owl:DatatypeProperty>
  <owl:DatatypeProperty rdf:about="http://example.org/onto/prop/google_cloudbuild_bitbucket_server_config_name">
    <rdfs:label>name</rdfs:label>
    <rdfs:comment>The resource name for the config.</rdfs:comment>
    <rdfs:domain rdf:resource="http://example.org/onto/class/google_cloudbuild_bitbucket_server_config"/>
    <rdfs:range rdf:resource="http://www.w3.org/2001/XMLSchema#string"/>
  </owl:DatatypeProperty>
  <owl:DatatypeProperty rdf:about="http://example.org/onto/prop/google_cloudbuild_bitbucket_server_config_peered_network">
    <rdfs:label>peered_network</rdfs:label>
    <rdfs:comment>The network to be used when reaching out to the Bitbucket Server instance. The VPC network must be enabled for private service connection.
This should be set if the Bitbucket Server instance is hosted on-premises and not reachable by public internet. If this field is left empty,
no network peering will occur and calls to the Bitbucket Server instance will be made over the public internet. Must be in the format
projects/{project}/global/networks/{network}, where {project} is a project number or id and {network} is the name of a VPC network in the project.</rdfs:comment>
    <rdfs:domain rdf:resource="http://example.org/onto/class/google_cloudbuild_bitbucket_server_config"/>
    <rdfs:range rdf:resource="http://www.w3.org/2001/XMLSchema#string"/>
  </owl:DatatypeProperty>
  <owl:DatatypeProperty rdf:about="http://example.org/onto/prop/google_cloudbuild_bitbucket_server_config_project">
    <rdfs:label>project</rdfs:label>
    <rdfs:domain rdf:resource="http://example.org/onto/class/google_cloudbuild_bitbucket_server_config"/>
    <rdfs:range rdf:resource="http://www.w3.org/2001/XMLSchema#string"/>
  </owl:DatatypeProperty>
  <owl:DatatypeProperty rdf:about="http://example.org/onto/prop/google_cloudbuild_bitbucket_server_config_ssl_ca">
    <rdfs:label>ssl_ca</rdfs:label>
    <rdfs:comment>SSL certificate to use for requests to Bitbucket Server. The format should be PEM format but the extension can be one of .pem, .cer, or .crt.</rdfs:comment>
    <rdfs:domain rdf:resource="http://example.org/onto/class/google_cloudbuild_bitbucket_server_config"/>
    <rdfs:range rdf:resource="http://www.w3.org/2001/XMLSchema#string"/>
  </owl:DatatypeProperty>
  <owl:DatatypeProperty rdf:about="http://example.org/onto/prop/google_cloudbuild_bitbucket_server_config_username">
    <rdfs:label>username</rdfs:label>
    <rdfs:comment>Username of the account Cloud Build will use on Bitbucket Server.</rdfs:comment>
    <rdfs:domain rdf:resource="http://example.org/onto/class/google_cloudbuild_bitbucket_server_config"/>
    <rdfs:range rdf:resource="http://www.w3.org/2001/XMLSchema#string"/>
  </owl:DatatypeProperty>
  <owl:DatatypeProperty rdf:about="http://example.org/onto/prop/google_cloudbuild_bitbucket_server_config_webhook_key">
    <rdfs:label>webhook_key</rdfs:label>
    <rdfs:comment>Output only. UUID included in webhook requests. The UUID is used to look up the corresponding config.</rdfs:comment>
    <rdfs:domain rdf:resource="http://example.org/onto/class/google_cloudbuild_bitbucket_server_config"/>
    <rdfs:range rdf:resource="http://www.w3.org/2001/XMLSchema#string"/>
  </owl:DatatypeProperty>
  <owl:DatatypeProperty rdf:about="http://example.org/onto/prop/google_cloudbuild_bitbucket_server_config_project_key">
    <rdfs:label>project_key</rdfs:label>
    <rdfs:comment>Identifier for the project storing the repository.</rdfs:comment>
    <rdfs:domain rdf:resource="http://example.org/onto/class/google_cloudbuild_bitbucket_server_config"/>
    <rdfs:range rdf:resource="http://www.w3.org/2001/XMLSchema#string"/>
  </owl:DatatypeProperty>
  <owl:DatatypeProperty rdf:about="http://example.org/onto/prop/google_cloudbuild_bitbucket_server_config_repo_slug">
    <rdfs:label>repo_slug</rdfs:label>
    <rdfs:comment>Identifier for the repository.</rdfs:comment>
    <rdfs:domain rdf:resource="http://example.org/onto/class/google_cloudbuild_bitbucket_server_config"/>
    <rdfs:range rdf:resource="http://www.w3.org/2001/XMLSchema#string"/>
  </owl:DatatypeProperty>
  <owl:DatatypeProperty rdf:about="http://example.org/onto/prop/google_cloudbuild_bitbucket_server_config_admin_access_token_version_name">
    <rdfs:label>admin_access_token_version_name</rdfs:label>
    <rdfs:comment>The resource name for the admin access token's secret version.</rdfs:comment>
    <rdfs:domain rdf:resource="http://example.org/onto/class/google_cloudbuild_bitbucket_server_config"/>
    <rdfs:range rdf:resource="http://www.w3.org/2001/XMLSchema#string"/>
  </owl:DatatypeProperty>
  <owl:DatatypeProperty rdf:about="http://example.org/onto/prop/google_cloudbuild_bitbucket_server_config_read_access_token_version_name">
    <rdfs:label>read_access_token_version_name</rdfs:label>
    <rdfs:comment>The resource name for the read access token's secret version.</rdfs:comment>
    <rdfs:domain rdf:resource="http://example.org/onto/class/google_cloudbuild_bitbucket_server_config"/>
    <rdfs:range rdf:resource="http://www.w3.org/2001/XMLSchema#string"/>
  </owl:DatatypeProperty>
  <owl:DatatypeProperty rdf:about="http://example.org/onto/prop/google_cloudbuild_bitbucket_server_config_webhook_secret_version_name">
    <rdfs:label>webhook_secret_version_name</rdfs:label>
    <rdfs:comment>Immutable. The resource name for the webhook secret's secret version. Once this field has been set, it cannot be changed.
Changing this field will result in deleting/ recreating the resource.</rdfs:comment>
    <rdfs:domain rdf:resource="http://example.org/onto/class/google_cloudbuild_bitbucket_server_config"/>
    <rdfs:range rdf:resource="http://www.w3.org/2001/XMLSchema#string"/>
  </owl:DatatypeProperty>
  <owl:DatatypeProperty rdf:about="http://example.org/onto/prop/google_cloudbuild_bitbucket_server_config_create">
    <rdfs:label>create</rdfs:label>
    <rdfs:domain rdf:resource="http://example.org/onto/class/google_cloudbuild_bitbucket_server_config"/>
    <rdfs:range rdf:resource="http://www.w3.org/2001/XMLSchema#string"/>
  </owl:DatatypeProperty>
  <owl:DatatypeProperty rdf:about="http://example.org/onto/prop/google_cloudbuild_bitbucket_server_config_delete">
    <rdfs:label>delete</rdfs:label>
    <rdfs:domain rdf:resource="http://example.org/onto/class/google_cloudbuild_bitbucket_server_config"/>
    <rdfs:range rdf:resource="http://www.w3.org/2001/XMLSchema#string"/>
  </owl:DatatypeProperty>
  <owl:DatatypeProperty rdf:about="http://example.org/onto/prop/google_cloudbuild_bitbucket_server_config_update">
    <rdfs:label>update</rdfs:label>
    <rdfs:domain rdf:resource="http://example.org/onto/class/google_cloudbuild_bitbucket_server_config"/>
    <rdfs:range rdf:resource="http://www.w3.org/2001/XMLSchema#string"/>
  </owl:DatatypeProperty>
</rdf:RDF>
