<?xml version="1.0" encoding="UTF-8"?>
<rdf:RDF
  xmlns:rdf="http://www.w3.org/1999/02/22-rdf-syntax-ns#"
  xmlns:rdfs="http://www.w3.org/2000/01/rdf-schema#"
  xmlns:owl="http://www.w3.org/2002/07/owl#"
  xmlns:xsd="http://www.w3.org/2001/XMLSchema#"
  xml:base="http://example.org/onto/">
  <owl:Class rdf:about="http://example.org/onto/class/google_dataplex_task">
    <rdfs:label>google_dataplex_task</rdfs:label>
    <rdfs:comment>#
#     ***     AUTO GENERATED CODE    ***    Type: MMv1     ***
#
# ----------------------------------------------------------------------------
#
#     This code is generated by Magic Modules using the following:
#
#     Configuration: https:#github.com/GoogleCloudPlatform/magic-modules/tree/main/mmv1/products/dataplex/Task.yaml
#     Template:      https:#github.com/GoogleCloudPlatform/magic-modules/tree/main/mmv1/templates/terraform/resource.html.markdown.tmpl
#
#     DO NOT EDIT this file directly. Any changes made to this file will be
#     overwritten during the next generation cycle.
#
# ----------------------------------------------------------------------------
subcategory: "Dataplex"
description: |-
  A Dataplex task represents the work that you want Dataplex to do on a schedule.
---</rdfs:comment>
  </owl:Class>
  <owl:DatatypeProperty rdf:about="http://example.org/onto/prop/google_dataplex_task_create_time">
    <rdfs:label>create_time</rdfs:label>
    <rdfs:comment>The time when the task was created.</rdfs:comment>
    <rdfs:domain rdf:resource="http://example.org/onto/class/google_dataplex_task"/>
    <rdfs:range rdf:resource="http://www.w3.org/2001/XMLSchema#string"/>
  </owl:DatatypeProperty>
  <owl:DatatypeProperty rdf:about="http://example.org/onto/prop/google_dataplex_task_description">
    <rdfs:label>description</rdfs:label>
    <rdfs:comment>User-provided description of the task.</rdfs:comment>
    <rdfs:domain rdf:resource="http://example.org/onto/class/google_dataplex_task"/>
    <rdfs:range rdf:resource="http://www.w3.org/2001/XMLSchema#string"/>
  </owl:DatatypeProperty>
  <owl:DatatypeProperty rdf:about="http://example.org/onto/prop/google_dataplex_task_display_name">
    <rdfs:label>display_name</rdfs:label>
    <rdfs:comment>User friendly display name.</rdfs:comment>
    <rdfs:domain rdf:resource="http://example.org/onto/class/google_dataplex_task"/>
    <rdfs:range rdf:resource="http://www.w3.org/2001/XMLSchema#string"/>
  </owl:DatatypeProperty>
  <owl:DatatypeProperty rdf:about="http://example.org/onto/prop/google_dataplex_task_effective_labels">
    <rdfs:label>effective_labels</rdfs:label>
    <rdfs:comment>All of labels (key/value pairs) present on the resource in GCP, including the labels configured through Terraform, other clients and services.</rdfs:comment>
    <rdfs:domain rdf:resource="http://example.org/onto/class/google_dataplex_task"/>
    <rdfs:range rdf:resource="http://www.w3.org/2001/XMLSchema#string"/>
  </owl:DatatypeProperty>
  <owl:DatatypeProperty rdf:about="http://example.org/onto/prop/google_dataplex_task_execution_status">
    <rdfs:label>execution_status</rdfs:label>
    <rdfs:comment>Configuration for the cluster</rdfs:comment>
    <rdfs:domain rdf:resource="http://example.org/onto/class/google_dataplex_task"/>
    <rdfs:range rdf:resource="http://www.w3.org/2001/XMLSchema#string"/>
  </owl:DatatypeProperty>
  <owl:DatatypeProperty rdf:about="http://example.org/onto/prop/google_dataplex_task_id">
    <rdfs:label>id</rdfs:label>
    <rdfs:domain rdf:resource="http://example.org/onto/class/google_dataplex_task"/>
    <rdfs:range rdf:resource="http://www.w3.org/2001/XMLSchema#string"/>
  </owl:DatatypeProperty>
  <owl:DatatypeProperty rdf:about="http://example.org/onto/prop/google_dataplex_task_labels">
    <rdfs:label>labels</rdfs:label>
    <rdfs:comment>User-defined labels for the task.


**Note**: This field is non-authoritative, and will only manage the labels present in your configuration.
Please refer to the field 'effective_labels' for all of the labels present on the resource.</rdfs:comment>
    <rdfs:domain rdf:resource="http://example.org/onto/class/google_dataplex_task"/>
    <rdfs:range rdf:resource="http://www.w3.org/2001/XMLSchema#string"/>
  </owl:DatatypeProperty>
  <owl:DatatypeProperty rdf:about="http://example.org/onto/prop/google_dataplex_task_lake">
    <rdfs:label>lake</rdfs:label>
    <rdfs:comment>The lake in which the task will be created in.</rdfs:comment>
    <rdfs:domain rdf:resource="http://example.org/onto/class/google_dataplex_task"/>
    <rdfs:range rdf:resource="http://www.w3.org/2001/XMLSchema#string"/>
  </owl:DatatypeProperty>
  <owl:DatatypeProperty rdf:about="http://example.org/onto/prop/google_dataplex_task_location">
    <rdfs:label>location</rdfs:label>
    <rdfs:comment>The location in which the task will be created in.</rdfs:comment>
    <rdfs:domain rdf:resource="http://example.org/onto/class/google_dataplex_task"/>
    <rdfs:range rdf:resource="http://www.w3.org/2001/XMLSchema#string"/>
  </owl:DatatypeProperty>
  <owl:DatatypeProperty rdf:about="http://example.org/onto/prop/google_dataplex_task_name">
    <rdfs:label>name</rdfs:label>
    <rdfs:comment>The relative resource name of the task, of the form: projects/{project_number}/locations/{locationId}/lakes/{lakeId}/ tasks/{name}.</rdfs:comment>
    <rdfs:domain rdf:resource="http://example.org/onto/class/google_dataplex_task"/>
    <rdfs:range rdf:resource="http://www.w3.org/2001/XMLSchema#string"/>
  </owl:DatatypeProperty>
  <owl:DatatypeProperty rdf:about="http://example.org/onto/prop/google_dataplex_task_project">
    <rdfs:label>project</rdfs:label>
    <rdfs:domain rdf:resource="http://example.org/onto/class/google_dataplex_task"/>
    <rdfs:range rdf:resource="http://www.w3.org/2001/XMLSchema#string"/>
  </owl:DatatypeProperty>
  <owl:DatatypeProperty rdf:about="http://example.org/onto/prop/google_dataplex_task_state">
    <rdfs:label>state</rdfs:label>
    <rdfs:comment>Current state of the task.</rdfs:comment>
    <rdfs:domain rdf:resource="http://example.org/onto/class/google_dataplex_task"/>
    <rdfs:range rdf:resource="http://www.w3.org/2001/XMLSchema#string"/>
  </owl:DatatypeProperty>
  <owl:DatatypeProperty rdf:about="http://example.org/onto/prop/google_dataplex_task_task_id">
    <rdfs:label>task_id</rdfs:label>
    <rdfs:comment>The task Id of the task.</rdfs:comment>
    <rdfs:domain rdf:resource="http://example.org/onto/class/google_dataplex_task"/>
    <rdfs:range rdf:resource="http://www.w3.org/2001/XMLSchema#string"/>
  </owl:DatatypeProperty>
  <owl:DatatypeProperty rdf:about="http://example.org/onto/prop/google_dataplex_task_terraform_labels">
    <rdfs:label>terraform_labels</rdfs:label>
    <rdfs:comment>The combination of labels configured directly on the resource
 and default labels configured on the provider.</rdfs:comment>
    <rdfs:domain rdf:resource="http://example.org/onto/class/google_dataplex_task"/>
    <rdfs:range rdf:resource="http://www.w3.org/2001/XMLSchema#string"/>
  </owl:DatatypeProperty>
  <owl:DatatypeProperty rdf:about="http://example.org/onto/prop/google_dataplex_task_uid">
    <rdfs:label>uid</rdfs:label>
    <rdfs:comment>System generated globally unique ID for the task. This ID will be different if the task is deleted and re-created with the same name.</rdfs:comment>
    <rdfs:domain rdf:resource="http://example.org/onto/class/google_dataplex_task"/>
    <rdfs:range rdf:resource="http://www.w3.org/2001/XMLSchema#string"/>
  </owl:DatatypeProperty>
  <owl:DatatypeProperty rdf:about="http://example.org/onto/prop/google_dataplex_task_update_time">
    <rdfs:label>update_time</rdfs:label>
    <rdfs:comment>The time when the task was last updated.</rdfs:comment>
    <rdfs:domain rdf:resource="http://example.org/onto/class/google_dataplex_task"/>
    <rdfs:range rdf:resource="http://www.w3.org/2001/XMLSchema#string"/>
  </owl:DatatypeProperty>
  <owl:DatatypeProperty rdf:about="http://example.org/onto/prop/google_dataplex_task_args">
    <rdfs:label>args</rdfs:label>
    <rdfs:comment>The arguments to pass to the task. The args can use placeholders of the format ${placeholder} as part of key/value string. These will be interpolated before passing the args to the driver. Currently supported placeholders: - ${taskId} - ${job_time} To pass positional args, set the key as TASK_ARGS. The value should be a comma-separated string of all the positional arguments. To use a delimiter other than comma, refer to https://cloud.google.com/sdk/gcloud/reference/topic/escaping. In case of other keys being present in the args, then TASK_ARGS will be passed as the last argument. An object containing a list of 'key': value pairs. Example: { 'name': 'wrench', 'mass': '1.3kg', 'count': '3' }.</rdfs:comment>
    <rdfs:domain rdf:resource="http://example.org/onto/class/google_dataplex_task"/>
    <rdfs:range rdf:resource="http://www.w3.org/2001/XMLSchema#string"/>
  </owl:DatatypeProperty>
  <owl:DatatypeProperty rdf:about="http://example.org/onto/prop/google_dataplex_task_kms_key">
    <rdfs:label>kms_key</rdfs:label>
    <rdfs:comment>The Cloud KMS key to use for encryption, of the form: projects/{project_number}/locations/{locationId}/keyRings/{key-ring-name}/cryptoKeys/{key-name}.</rdfs:comment>
    <rdfs:domain rdf:resource="http://example.org/onto/class/google_dataplex_task"/>
    <rdfs:range rdf:resource="http://www.w3.org/2001/XMLSchema#string"/>
  </owl:DatatypeProperty>
  <owl:DatatypeProperty rdf:about="http://example.org/onto/prop/google_dataplex_task_max_job_execution_lifetime">
    <rdfs:label>max_job_execution_lifetime</rdfs:label>
    <rdfs:comment>The maximum duration after which the job execution is expired. A duration in seconds with up to nine fractional digits, ending with 's'. Example: '3.5s'.</rdfs:comment>
    <rdfs:domain rdf:resource="http://example.org/onto/class/google_dataplex_task"/>
    <rdfs:range rdf:resource="http://www.w3.org/2001/XMLSchema#string"/>
  </owl:DatatypeProperty>
  <owl:DatatypeProperty rdf:about="http://example.org/onto/prop/google_dataplex_task_project">
    <rdfs:label>project</rdfs:label>
    <rdfs:comment>The project in which jobs are run. By default, the project containing the Lake is used. If a project is provided, the ExecutionSpec.service_account must belong to this project.</rdfs:comment>
    <rdfs:domain rdf:resource="http://example.org/onto/class/google_dataplex_task"/>
    <rdfs:range rdf:resource="http://www.w3.org/2001/XMLSchema#string"/>
  </owl:DatatypeProperty>
  <owl:DatatypeProperty rdf:about="http://example.org/onto/prop/google_dataplex_task_service_account">
    <rdfs:label>service_account</rdfs:label>
    <rdfs:comment>Service account to use to execute a task. If not provided, the default Compute service account for the project is used.</rdfs:comment>
    <rdfs:domain rdf:resource="http://example.org/onto/class/google_dataplex_task"/>
    <rdfs:range rdf:resource="http://www.w3.org/2001/XMLSchema#string"/>
  </owl:DatatypeProperty>
  <owl:DatatypeProperty rdf:about="http://example.org/onto/prop/google_dataplex_task_archive_uris">
    <rdfs:label>archive_uris</rdfs:label>
    <rdfs:comment>Cloud Storage URIs of archives to be extracted into the working directory of each executor. Supported file types: .jar, .tar, .tar.gz, .tgz, and .zip.</rdfs:comment>
    <rdfs:domain rdf:resource="http://example.org/onto/class/google_dataplex_task"/>
    <rdfs:range rdf:resource="http://www.w3.org/2001/XMLSchema#string"/>
  </owl:DatatypeProperty>
  <owl:DatatypeProperty rdf:about="http://example.org/onto/prop/google_dataplex_task_file_uris">
    <rdfs:label>file_uris</rdfs:label>
    <rdfs:comment>Cloud Storage URIs of files to be placed in the working directory of each executor.</rdfs:comment>
    <rdfs:domain rdf:resource="http://example.org/onto/class/google_dataplex_task"/>
    <rdfs:range rdf:resource="http://www.w3.org/2001/XMLSchema#string"/>
  </owl:DatatypeProperty>
  <owl:DatatypeProperty rdf:about="http://example.org/onto/prop/google_dataplex_task_notebook">
    <rdfs:label>notebook</rdfs:label>
    <rdfs:comment>Path to input notebook. This can be the Cloud Storage URI of the notebook file or the path to a Notebook Content. The execution args are accessible as environment variables (TASK_key=value).</rdfs:comment>
    <rdfs:domain rdf:resource="http://example.org/onto/class/google_dataplex_task"/>
    <rdfs:range rdf:resource="http://www.w3.org/2001/XMLSchema#string"/>
  </owl:DatatypeProperty>
  <owl:DatatypeProperty rdf:about="http://example.org/onto/prop/google_dataplex_task_executors_count">
    <rdfs:label>executors_count</rdfs:label>
    <rdfs:comment>Total number of job executors. Executor Count should be between 2 and 100. [Default=2]</rdfs:comment>
    <rdfs:domain rdf:resource="http://example.org/onto/class/google_dataplex_task"/>
    <rdfs:range rdf:resource="http://www.w3.org/2001/XMLSchema#string"/>
  </owl:DatatypeProperty>
  <owl:DatatypeProperty rdf:about="http://example.org/onto/prop/google_dataplex_task_max_executors_count">
    <rdfs:label>max_executors_count</rdfs:label>
    <rdfs:comment>Max configurable executors. If maxExecutorsCount > executorsCount, then auto-scaling is enabled. Max Executor Count should be between 2 and 1000. [Default=1000]</rdfs:comment>
    <rdfs:domain rdf:resource="http://example.org/onto/class/google_dataplex_task"/>
    <rdfs:range rdf:resource="http://www.w3.org/2001/XMLSchema#string"/>
  </owl:DatatypeProperty>
  <owl:DatatypeProperty rdf:about="http://example.org/onto/prop/google_dataplex_task_image">
    <rdfs:label>image</rdfs:label>
    <rdfs:comment>Container image to use.</rdfs:comment>
    <rdfs:domain rdf:resource="http://example.org/onto/class/google_dataplex_task"/>
    <rdfs:range rdf:resource="http://www.w3.org/2001/XMLSchema#string"/>
  </owl:DatatypeProperty>
  <owl:DatatypeProperty rdf:about="http://example.org/onto/prop/google_dataplex_task_java_jars">
    <rdfs:label>java_jars</rdfs:label>
    <rdfs:comment>A list of Java JARS to add to the classpath. Valid input includes Cloud Storage URIs to Jar binaries. For example, gs://bucket-name/my/path/to/file.jar</rdfs:comment>
    <rdfs:domain rdf:resource="http://example.org/onto/class/google_dataplex_task"/>
    <rdfs:range rdf:resource="http://www.w3.org/2001/XMLSchema#string"/>
  </owl:DatatypeProperty>
  <owl:DatatypeProperty rdf:about="http://example.org/onto/prop/google_dataplex_task_properties">
    <rdfs:label>properties</rdfs:label>
    <rdfs:comment>Override to common configuration of open source components installed on the Dataproc cluster. The properties to set on daemon config files. Property keys are specified in prefix:property format, for example core:hadoop.tmp.dir. For more information, see Cluster properties.</rdfs:comment>
    <rdfs:domain rdf:resource="http://example.org/onto/class/google_dataplex_task"/>
    <rdfs:range rdf:resource="http://www.w3.org/2001/XMLSchema#string"/>
  </owl:DatatypeProperty>
  <owl:DatatypeProperty rdf:about="http://example.org/onto/prop/google_dataplex_task_python_packages">
    <rdfs:label>python_packages</rdfs:label>
    <rdfs:comment>A list of python packages to be installed. Valid formats include Cloud Storage URI to a PIP installable library. For example, gs://bucket-name/my/path/to/lib.tar.gz</rdfs:comment>
    <rdfs:domain rdf:resource="http://example.org/onto/class/google_dataplex_task"/>
    <rdfs:range rdf:resource="http://www.w3.org/2001/XMLSchema#string"/>
  </owl:DatatypeProperty>
  <owl:DatatypeProperty rdf:about="http://example.org/onto/prop/google_dataplex_task_network">
    <rdfs:label>network</rdfs:label>
    <rdfs:comment>The Cloud VPC network in which the job is run. By default, the Cloud VPC network named Default within the project is used.</rdfs:comment>
    <rdfs:domain rdf:resource="http://example.org/onto/class/google_dataplex_task"/>
    <rdfs:range rdf:resource="http://www.w3.org/2001/XMLSchema#string"/>
  </owl:DatatypeProperty>
  <owl:DatatypeProperty rdf:about="http://example.org/onto/prop/google_dataplex_task_network_tags">
    <rdfs:label>network_tags</rdfs:label>
    <rdfs:comment>List of network tags to apply to the job.</rdfs:comment>
    <rdfs:domain rdf:resource="http://example.org/onto/class/google_dataplex_task"/>
    <rdfs:range rdf:resource="http://www.w3.org/2001/XMLSchema#string"/>
  </owl:DatatypeProperty>
  <owl:DatatypeProperty rdf:about="http://example.org/onto/prop/google_dataplex_task_sub_network">
    <rdfs:label>sub_network</rdfs:label>
    <rdfs:comment>The Cloud VPC sub-network in which the job is run.</rdfs:comment>
    <rdfs:domain rdf:resource="http://example.org/onto/class/google_dataplex_task"/>
    <rdfs:range rdf:resource="http://www.w3.org/2001/XMLSchema#string"/>
  </owl:DatatypeProperty>
  <owl:DatatypeProperty rdf:about="http://example.org/onto/prop/google_dataplex_task_archive_uris">
    <rdfs:label>archive_uris</rdfs:label>
    <rdfs:comment>Cloud Storage URIs of archives to be extracted into the working directory of each executor. Supported file types: .jar, .tar, .tar.gz, .tgz, and .zip.</rdfs:comment>
    <rdfs:domain rdf:resource="http://example.org/onto/class/google_dataplex_task"/>
    <rdfs:range rdf:resource="http://www.w3.org/2001/XMLSchema#string"/>
  </owl:DatatypeProperty>
  <owl:DatatypeProperty rdf:about="http://example.org/onto/prop/google_dataplex_task_file_uris">
    <rdfs:label>file_uris</rdfs:label>
    <rdfs:comment>Cloud Storage URIs of files to be placed in the working directory of each executor.</rdfs:comment>
    <rdfs:domain rdf:resource="http://example.org/onto/class/google_dataplex_task"/>
    <rdfs:range rdf:resource="http://www.w3.org/2001/XMLSchema#string"/>
  </owl:DatatypeProperty>
  <owl:DatatypeProperty rdf:about="http://example.org/onto/prop/google_dataplex_task_main_class">
    <rdfs:label>main_class</rdfs:label>
    <rdfs:comment>The name of the driver's main class. The jar file that contains the class must be in the default CLASSPATH or specified in jar_file_uris. The execution args are passed in as a sequence of named process arguments (--key=value).</rdfs:comment>
    <rdfs:domain rdf:resource="http://example.org/onto/class/google_dataplex_task"/>
    <rdfs:range rdf:resource="http://www.w3.org/2001/XMLSchema#string"/>
  </owl:DatatypeProperty>
  <owl:DatatypeProperty rdf:about="http://example.org/onto/prop/google_dataplex_task_main_jar_file_uri">
    <rdfs:label>main_jar_file_uri</rdfs:label>
    <rdfs:comment>The Cloud Storage URI of the jar file that contains the main class. The execution args are passed in as a sequence of named process arguments (--key=value).</rdfs:comment>
    <rdfs:domain rdf:resource="http://example.org/onto/class/google_dataplex_task"/>
    <rdfs:range rdf:resource="http://www.w3.org/2001/XMLSchema#string"/>
  </owl:DatatypeProperty>
  <owl:DatatypeProperty rdf:about="http://example.org/onto/prop/google_dataplex_task_python_script_file">
    <rdfs:label>python_script_file</rdfs:label>
    <rdfs:comment>The Gcloud Storage URI of the main Python file to use as the driver. Must be a .py file. The execution args are passed in as a sequence of named process arguments (--key=value).</rdfs:comment>
    <rdfs:domain rdf:resource="http://example.org/onto/class/google_dataplex_task"/>
    <rdfs:range rdf:resource="http://www.w3.org/2001/XMLSchema#string"/>
  </owl:DatatypeProperty>
  <owl:DatatypeProperty rdf:about="http://example.org/onto/prop/google_dataplex_task_sql_script">
    <rdfs:label>sql_script</rdfs:label>
    <rdfs:comment>The query text. The execution args are used to declare a set of script variables (set key='value';).</rdfs:comment>
    <rdfs:domain rdf:resource="http://example.org/onto/class/google_dataplex_task"/>
    <rdfs:range rdf:resource="http://www.w3.org/2001/XMLSchema#string"/>
  </owl:DatatypeProperty>
  <owl:DatatypeProperty rdf:about="http://example.org/onto/prop/google_dataplex_task_sql_script_file">
    <rdfs:label>sql_script_file</rdfs:label>
    <rdfs:comment>A reference to a query file. This can be the Cloud Storage URI of the query file or it can the path to a SqlScript Content. The execution args are used to declare a set of script variables (set key='value';).</rdfs:comment>
    <rdfs:domain rdf:resource="http://example.org/onto/class/google_dataplex_task"/>
    <rdfs:range rdf:resource="http://www.w3.org/2001/XMLSchema#string"/>
  </owl:DatatypeProperty>
  <owl:DatatypeProperty rdf:about="http://example.org/onto/prop/google_dataplex_task_executors_count">
    <rdfs:label>executors_count</rdfs:label>
    <rdfs:comment>Total number of job executors. Executor Count should be between 2 and 100. [Default=2]</rdfs:comment>
    <rdfs:domain rdf:resource="http://example.org/onto/class/google_dataplex_task"/>
    <rdfs:range rdf:resource="http://www.w3.org/2001/XMLSchema#string"/>
  </owl:DatatypeProperty>
  <owl:DatatypeProperty rdf:about="http://example.org/onto/prop/google_dataplex_task_max_executors_count">
    <rdfs:label>max_executors_count</rdfs:label>
    <rdfs:comment>Max configurable executors. If maxExecutorsCount > executorsCount, then auto-scaling is enabled. Max Executor Count should be between 2 and 1000. [Default=1000]</rdfs:comment>
    <rdfs:domain rdf:resource="http://example.org/onto/class/google_dataplex_task"/>
    <rdfs:range rdf:resource="http://www.w3.org/2001/XMLSchema#string"/>
  </owl:DatatypeProperty>
  <owl:DatatypeProperty rdf:about="http://example.org/onto/prop/google_dataplex_task_image">
    <rdfs:label>image</rdfs:label>
    <rdfs:comment>Container image to use.</rdfs:comment>
    <rdfs:domain rdf:resource="http://example.org/onto/class/google_dataplex_task"/>
    <rdfs:range rdf:resource="http://www.w3.org/2001/XMLSchema#string"/>
  </owl:DatatypeProperty>
  <owl:DatatypeProperty rdf:about="http://example.org/onto/prop/google_dataplex_task_java_jars">
    <rdfs:label>java_jars</rdfs:label>
    <rdfs:comment>A list of Java JARS to add to the classpath. Valid input includes Cloud Storage URIs to Jar binaries. For example, gs://bucket-name/my/path/to/file.jar</rdfs:comment>
    <rdfs:domain rdf:resource="http://example.org/onto/class/google_dataplex_task"/>
    <rdfs:range rdf:resource="http://www.w3.org/2001/XMLSchema#string"/>
  </owl:DatatypeProperty>
  <owl:DatatypeProperty rdf:about="http://example.org/onto/prop/google_dataplex_task_properties">
    <rdfs:label>properties</rdfs:label>
    <rdfs:comment>Override to common configuration of open source components installed on the Dataproc cluster. The properties to set on daemon config files. Property keys are specified in prefix:property format, for example core:hadoop.tmp.dir. For more information, see Cluster properties.</rdfs:comment>
    <rdfs:domain rdf:resource="http://example.org/onto/class/google_dataplex_task"/>
    <rdfs:range rdf:resource="http://www.w3.org/2001/XMLSchema#string"/>
  </owl:DatatypeProperty>
  <owl:DatatypeProperty rdf:about="http://example.org/onto/prop/google_dataplex_task_python_packages">
    <rdfs:label>python_packages</rdfs:label>
    <rdfs:comment>A list of python packages to be installed. Valid formats include Cloud Storage URI to a PIP installable library. For example, gs://bucket-name/my/path/to/lib.tar.gz</rdfs:comment>
    <rdfs:domain rdf:resource="http://example.org/onto/class/google_dataplex_task"/>
    <rdfs:range rdf:resource="http://www.w3.org/2001/XMLSchema#string"/>
  </owl:DatatypeProperty>
  <owl:DatatypeProperty rdf:about="http://example.org/onto/prop/google_dataplex_task_network">
    <rdfs:label>network</rdfs:label>
    <rdfs:comment>The Cloud VPC network in which the job is run. By default, the Cloud VPC network named Default within the project is used.</rdfs:comment>
    <rdfs:domain rdf:resource="http://example.org/onto/class/google_dataplex_task"/>
    <rdfs:range rdf:resource="http://www.w3.org/2001/XMLSchema#string"/>
  </owl:DatatypeProperty>
  <owl:DatatypeProperty rdf:about="http://example.org/onto/prop/google_dataplex_task_network_tags">
    <rdfs:label>network_tags</rdfs:label>
    <rdfs:comment>List of network tags to apply to the job.</rdfs:comment>
    <rdfs:domain rdf:resource="http://example.org/onto/class/google_dataplex_task"/>
    <rdfs:range rdf:resource="http://www.w3.org/2001/XMLSchema#string"/>
  </owl:DatatypeProperty>
  <owl:DatatypeProperty rdf:about="http://example.org/onto/prop/google_dataplex_task_sub_network">
    <rdfs:label>sub_network</rdfs:label>
    <rdfs:comment>The Cloud VPC sub-network in which the job is run.</rdfs:comment>
    <rdfs:domain rdf:resource="http://example.org/onto/class/google_dataplex_task"/>
    <rdfs:range rdf:resource="http://www.w3.org/2001/XMLSchema#string"/>
  </owl:DatatypeProperty>
  <owl:DatatypeProperty rdf:about="http://example.org/onto/prop/google_dataplex_task_create">
    <rdfs:label>create</rdfs:label>
    <rdfs:domain rdf:resource="http://example.org/onto/class/google_dataplex_task"/>
    <rdfs:range rdf:resource="http://www.w3.org/2001/XMLSchema#string"/>
  </owl:DatatypeProperty>
  <owl:DatatypeProperty rdf:about="http://example.org/onto/prop/google_dataplex_task_delete">
    <rdfs:label>delete</rdfs:label>
    <rdfs:domain rdf:resource="http://example.org/onto/class/google_dataplex_task"/>
    <rdfs:range rdf:resource="http://www.w3.org/2001/XMLSchema#string"/>
  </owl:DatatypeProperty>
  <owl:DatatypeProperty rdf:about="http://example.org/onto/prop/google_dataplex_task_update">
    <rdfs:label>update</rdfs:label>
    <rdfs:domain rdf:resource="http://example.org/onto/class/google_dataplex_task"/>
    <rdfs:range rdf:resource="http://www.w3.org/2001/XMLSchema#string"/>
  </owl:DatatypeProperty>
  <owl:DatatypeProperty rdf:about="http://example.org/onto/prop/google_dataplex_task_disabled">
    <rdfs:label>disabled</rdfs:label>
    <rdfs:comment>Prevent the task from executing. This does not cancel already running tasks. It is intended to temporarily disable RECURRING tasks.</rdfs:comment>
    <rdfs:domain rdf:resource="http://example.org/onto/class/google_dataplex_task"/>
    <rdfs:range rdf:resource="http://www.w3.org/2001/XMLSchema#string"/>
  </owl:DatatypeProperty>
  <owl:DatatypeProperty rdf:about="http://example.org/onto/prop/google_dataplex_task_max_retries">
    <rdfs:label>max_retries</rdfs:label>
    <rdfs:comment>Number of retry attempts before aborting. Set to zero to never attempt to retry a failed task.</rdfs:comment>
    <rdfs:domain rdf:resource="http://example.org/onto/class/google_dataplex_task"/>
    <rdfs:range rdf:resource="http://www.w3.org/2001/XMLSchema#string"/>
  </owl:DatatypeProperty>
  <owl:DatatypeProperty rdf:about="http://example.org/onto/prop/google_dataplex_task_schedule">
    <rdfs:label>schedule</rdfs:label>
    <rdfs:comment>Cron schedule (https://en.wikipedia.org/wiki/Cron) for running tasks periodically. To explicitly set a timezone to the cron tab, apply a prefix in the cron tab: 'CRON_TZ=${IANA_TIME_ZONE}' or 'TZ=${IANA_TIME_ZONE}'. The ${IANA_TIME_ZONE} may only be a valid string from IANA time zone database. For example, CRON_TZ=America/New_York 1 * * * *, or TZ=America/New_York 1 * * * *. This field is required for RECURRING tasks.</rdfs:comment>
    <rdfs:domain rdf:resource="http://example.org/onto/class/google_dataplex_task"/>
    <rdfs:range rdf:resource="http://www.w3.org/2001/XMLSchema#string"/>
  </owl:DatatypeProperty>
  <owl:DatatypeProperty rdf:about="http://example.org/onto/prop/google_dataplex_task_start_time">
    <rdfs:label>start_time</rdfs:label>
    <rdfs:comment>The first run of the task will be after this time. If not specified, the task will run shortly after being submitted if ON_DEMAND and based on the schedule if RECURRING.</rdfs:comment>
    <rdfs:domain rdf:resource="http://example.org/onto/class/google_dataplex_task"/>
    <rdfs:range rdf:resource="http://www.w3.org/2001/XMLSchema#string"/>
  </owl:DatatypeProperty>
  <owl:DatatypeProperty rdf:about="http://example.org/onto/prop/google_dataplex_task_type">
    <rdfs:label>type</rdfs:label>
    <rdfs:comment>Trigger type of the user-specified Task Possible values: ["ON_DEMAND", "RECURRING"]</rdfs:comment>
    <rdfs:domain rdf:resource="http://example.org/onto/class/google_dataplex_task"/>
    <rdfs:range rdf:resource="http://www.w3.org/2001/XMLSchema#string"/>
  </owl:DatatypeProperty>
</rdf:RDF>
