<?xml version="1.0" encoding="UTF-8"?>
<rdf:RDF
  xmlns:rdf="http://www.w3.org/1999/02/22-rdf-syntax-ns#"
  xmlns:rdfs="http://www.w3.org/2000/01/rdf-schema#"
  xmlns:owl="http://www.w3.org/2002/07/owl#"
  xmlns:xsd="http://www.w3.org/2001/XMLSchema#"
  xml:base="http://example.org/onto/">
  <owl:Class rdf:about="http://example.org/onto/class/google_redis_cluster_user_created_connections">
    <rdfs:label>google_redis_cluster_user_created_connections</rdfs:label>
    <rdfs:comment>#
#     ***     AUTO GENERATED CODE    ***    Type: MMv1     ***
#
# ----------------------------------------------------------------------------
#
#     This code is generated by Magic Modules using the following:
#
#     Configuration: https:#github.com/GoogleCloudPlatform/magic-modules/tree/main/mmv1/products/redis/ClusterUserCreatedConnections.yaml
#     Template:      https:#github.com/GoogleCloudPlatform/magic-modules/tree/main/mmv1/templates/terraform/resource.html.markdown.tmpl
#
#     DO NOT EDIT this file directly. Any changes made to this file will be
#     overwritten during the next generation cycle.
#
# ----------------------------------------------------------------------------
subcategory: "Memorystore (Redis)"
description: |-
  Manages user created connections for Redis cluster
---</rdfs:comment>
  </owl:Class>
  <owl:DatatypeProperty rdf:about="http://example.org/onto/prop/google_redis_cluster_user_created_connections_id">
    <rdfs:label>id</rdfs:label>
    <rdfs:domain rdf:resource="http://example.org/onto/class/google_redis_cluster_user_created_connections"/>
    <rdfs:range rdf:resource="http://www.w3.org/2001/XMLSchema#string"/>
  </owl:DatatypeProperty>
  <owl:DatatypeProperty rdf:about="http://example.org/onto/prop/google_redis_cluster_user_created_connections_name">
    <rdfs:label>name</rdfs:label>
    <rdfs:comment>The name of the Redis cluster these endpoints should be added to.</rdfs:comment>
    <rdfs:domain rdf:resource="http://example.org/onto/class/google_redis_cluster_user_created_connections"/>
    <rdfs:range rdf:resource="http://www.w3.org/2001/XMLSchema#string"/>
  </owl:DatatypeProperty>
  <owl:DatatypeProperty rdf:about="http://example.org/onto/prop/google_redis_cluster_user_created_connections_project">
    <rdfs:label>project</rdfs:label>
    <rdfs:domain rdf:resource="http://example.org/onto/class/google_redis_cluster_user_created_connections"/>
    <rdfs:range rdf:resource="http://www.w3.org/2001/XMLSchema#string"/>
  </owl:DatatypeProperty>
  <owl:DatatypeProperty rdf:about="http://example.org/onto/prop/google_redis_cluster_user_created_connections_region">
    <rdfs:label>region</rdfs:label>
    <rdfs:comment>The name of the region of the Redis cluster these endpoints should be added to.</rdfs:comment>
    <rdfs:domain rdf:resource="http://example.org/onto/class/google_redis_cluster_user_created_connections"/>
    <rdfs:range rdf:resource="http://www.w3.org/2001/XMLSchema#string"/>
  </owl:DatatypeProperty>
  <owl:DatatypeProperty rdf:about="http://example.org/onto/prop/google_redis_cluster_user_created_connections_address">
    <rdfs:label>address</rdfs:label>
    <rdfs:comment>The IP allocated on the consumer network for the PSC forwarding rule.</rdfs:comment>
    <rdfs:domain rdf:resource="http://example.org/onto/class/google_redis_cluster_user_created_connections"/>
    <rdfs:range rdf:resource="http://www.w3.org/2001/XMLSchema#string"/>
  </owl:DatatypeProperty>
  <owl:DatatypeProperty rdf:about="http://example.org/onto/prop/google_redis_cluster_user_created_connections_connection_type">
    <rdfs:label>connection_type</rdfs:label>
    <rdfs:comment>Output Only. Type of a PSC Connection. 
 Possible values:
 CONNECTION_TYPE_DISCOVERY 
 CONNECTION_TYPE_PRIMARY 
 CONNECTION_TYPE_READER</rdfs:comment>
    <rdfs:domain rdf:resource="http://example.org/onto/class/google_redis_cluster_user_created_connections"/>
    <rdfs:range rdf:resource="http://www.w3.org/2001/XMLSchema#string"/>
  </owl:DatatypeProperty>
  <owl:DatatypeProperty rdf:about="http://example.org/onto/prop/google_redis_cluster_user_created_connections_forwarding_rule">
    <rdfs:label>forwarding_rule</rdfs:label>
    <rdfs:comment>The URI of the consumer side forwarding rule.
Format:
projects/{project}/regions/{region}/forwardingRules/{forwarding_rule}</rdfs:comment>
    <rdfs:domain rdf:resource="http://example.org/onto/class/google_redis_cluster_user_created_connections"/>
    <rdfs:range rdf:resource="http://www.w3.org/2001/XMLSchema#string"/>
  </owl:DatatypeProperty>
  <owl:DatatypeProperty rdf:about="http://example.org/onto/prop/google_redis_cluster_user_created_connections_network">
    <rdfs:label>network</rdfs:label>
    <rdfs:comment>The consumer network where the IP address resides, in the form of
projects/{project_id}/global/networks/{network_id}.</rdfs:comment>
    <rdfs:domain rdf:resource="http://example.org/onto/class/google_redis_cluster_user_created_connections"/>
    <rdfs:range rdf:resource="http://www.w3.org/2001/XMLSchema#string"/>
  </owl:DatatypeProperty>
  <owl:DatatypeProperty rdf:about="http://example.org/onto/prop/google_redis_cluster_user_created_connections_project_id">
    <rdfs:label>project_id</rdfs:label>
    <rdfs:comment>The consumer project_id where the forwarding rule is created from.</rdfs:comment>
    <rdfs:domain rdf:resource="http://example.org/onto/class/google_redis_cluster_user_created_connections"/>
    <rdfs:range rdf:resource="http://www.w3.org/2001/XMLSchema#string"/>
  </owl:DatatypeProperty>
  <owl:DatatypeProperty rdf:about="http://example.org/onto/prop/google_redis_cluster_user_created_connections_psc_connection_id">
    <rdfs:label>psc_connection_id</rdfs:label>
    <rdfs:comment>The PSC connection id of the forwarding rule connected to the
service attachment.</rdfs:comment>
    <rdfs:domain rdf:resource="http://example.org/onto/class/google_redis_cluster_user_created_connections"/>
    <rdfs:range rdf:resource="http://www.w3.org/2001/XMLSchema#string"/>
  </owl:DatatypeProperty>
  <owl:DatatypeProperty rdf:about="http://example.org/onto/prop/google_redis_cluster_user_created_connections_psc_connection_status">
    <rdfs:label>psc_connection_status</rdfs:label>
    <rdfs:comment>Output Only. The status of the PSC connection: whether a connection exists and ACTIVE or it no longer exists. 
 Possible values:
 ACTIVE 
 NOT_FOUND</rdfs:comment>
    <rdfs:domain rdf:resource="http://example.org/onto/class/google_redis_cluster_user_created_connections"/>
    <rdfs:range rdf:resource="http://www.w3.org/2001/XMLSchema#string"/>
  </owl:DatatypeProperty>
  <owl:DatatypeProperty rdf:about="http://example.org/onto/prop/google_redis_cluster_user_created_connections_service_attachment">
    <rdfs:label>service_attachment</rdfs:label>
    <rdfs:comment>The service attachment which is the target of the PSC connection, in the form of projects/{project-id}/regions/{region}/serviceAttachments/{service-attachment-id}.</rdfs:comment>
    <rdfs:domain rdf:resource="http://example.org/onto/class/google_redis_cluster_user_created_connections"/>
    <rdfs:range rdf:resource="http://www.w3.org/2001/XMLSchema#string"/>
  </owl:DatatypeProperty>
  <owl:DatatypeProperty rdf:about="http://example.org/onto/prop/google_redis_cluster_user_created_connections_create">
    <rdfs:label>create</rdfs:label>
    <rdfs:domain rdf:resource="http://example.org/onto/class/google_redis_cluster_user_created_connections"/>
    <rdfs:range rdf:resource="http://www.w3.org/2001/XMLSchema#string"/>
  </owl:DatatypeProperty>
  <owl:DatatypeProperty rdf:about="http://example.org/onto/prop/google_redis_cluster_user_created_connections_delete">
    <rdfs:label>delete</rdfs:label>
    <rdfs:domain rdf:resource="http://example.org/onto/class/google_redis_cluster_user_created_connections"/>
    <rdfs:range rdf:resource="http://www.w3.org/2001/XMLSchema#string"/>
  </owl:DatatypeProperty>
  <owl:DatatypeProperty rdf:about="http://example.org/onto/prop/google_redis_cluster_user_created_connections_update">
    <rdfs:label>update</rdfs:label>
    <rdfs:domain rdf:resource="http://example.org/onto/class/google_redis_cluster_user_created_connections"/>
    <rdfs:range rdf:resource="http://www.w3.org/2001/XMLSchema#string"/>
  </owl:DatatypeProperty>
</rdf:RDF>
