<?xml version="1.0" encoding="UTF-8"?>
<rdf:RDF
  xmlns:rdf="http://www.w3.org/1999/02/22-rdf-syntax-ns#"
  xmlns:rdfs="http://www.w3.org/2000/01/rdf-schema#"
  xmlns:owl="http://www.w3.org/2002/07/owl#"
  xmlns:xsd="http://www.w3.org/2001/XMLSchema#"
  xml:base="http://example.org/onto/">
  <owl:Class rdf:about="http://example.org/onto/class/google_dialogflow_cx_tool">
    <rdfs:label>google_dialogflow_cx_tool</rdfs:label>
    <rdfs:comment>#
#     ***     AUTO GENERATED CODE    ***    Type: MMv1     ***
#
# ----------------------------------------------------------------------------
#
#     This code is generated by Magic Modules using the following:
#
#     Configuration: https:#github.com/GoogleCloudPlatform/magic-modules/tree/main/mmv1/products/dialogflowcx/Tool.yaml
#     Template:      https:#github.com/GoogleCloudPlatform/magic-modules/tree/main/mmv1/templates/terraform/resource.html.markdown.tmpl
#
#     DO NOT EDIT this file directly. Any changes made to this file will be
#     overwritten during the next generation cycle.
#
# ----------------------------------------------------------------------------
subcategory: "Dialogflow CX"
description: |-
  A tool provides a list of actions which are available to the Playbook to attain its goal.
---</rdfs:comment>
  </owl:Class>
  <owl:DatatypeProperty rdf:about="http://example.org/onto/prop/google_dialogflow_cx_tool_description">
    <rdfs:label>description</rdfs:label>
    <rdfs:comment>High level description of the Tool and its usage.</rdfs:comment>
    <rdfs:domain rdf:resource="http://example.org/onto/class/google_dialogflow_cx_tool"/>
    <rdfs:range rdf:resource="http://www.w3.org/2001/XMLSchema#string"/>
  </owl:DatatypeProperty>
  <owl:DatatypeProperty rdf:about="http://example.org/onto/prop/google_dialogflow_cx_tool_display_name">
    <rdfs:label>display_name</rdfs:label>
    <rdfs:comment>The human-readable name of the tool, unique within the agent.</rdfs:comment>
    <rdfs:domain rdf:resource="http://example.org/onto/class/google_dialogflow_cx_tool"/>
    <rdfs:range rdf:resource="http://www.w3.org/2001/XMLSchema#string"/>
  </owl:DatatypeProperty>
  <owl:DatatypeProperty rdf:about="http://example.org/onto/prop/google_dialogflow_cx_tool_id">
    <rdfs:label>id</rdfs:label>
    <rdfs:domain rdf:resource="http://example.org/onto/class/google_dialogflow_cx_tool"/>
    <rdfs:range rdf:resource="http://www.w3.org/2001/XMLSchema#string"/>
  </owl:DatatypeProperty>
  <owl:DatatypeProperty rdf:about="http://example.org/onto/prop/google_dialogflow_cx_tool_name">
    <rdfs:label>name</rdfs:label>
    <rdfs:comment>The unique identifier of the Tool.
Format: projects/<Project ID>/locations/<Location ID>/agents/<Agent ID>/tools/<Tool ID>.</rdfs:comment>
    <rdfs:domain rdf:resource="http://example.org/onto/class/google_dialogflow_cx_tool"/>
    <rdfs:range rdf:resource="http://www.w3.org/2001/XMLSchema#string"/>
  </owl:DatatypeProperty>
  <owl:DatatypeProperty rdf:about="http://example.org/onto/prop/google_dialogflow_cx_tool_parent">
    <rdfs:label>parent</rdfs:label>
    <rdfs:comment>The agent to create a Tool for.
Format: projects/<Project ID>/locations/<Location ID>/agents/<Agent ID>.</rdfs:comment>
    <rdfs:domain rdf:resource="http://example.org/onto/class/google_dialogflow_cx_tool"/>
    <rdfs:range rdf:resource="http://www.w3.org/2001/XMLSchema#string"/>
  </owl:DatatypeProperty>
  <owl:DatatypeProperty rdf:about="http://example.org/onto/prop/google_dialogflow_cx_tool_tool_type">
    <rdfs:label>tool_type</rdfs:label>
    <rdfs:comment>The tool type.</rdfs:comment>
    <rdfs:domain rdf:resource="http://example.org/onto/class/google_dialogflow_cx_tool"/>
    <rdfs:range rdf:resource="http://www.w3.org/2001/XMLSchema#string"/>
  </owl:DatatypeProperty>
  <owl:DatatypeProperty rdf:about="http://example.org/onto/prop/google_dialogflow_cx_tool_data_store">
    <rdfs:label>data_store</rdfs:label>
    <rdfs:comment>The full name of the referenced data store. Formats: projects/{project}/locations/{location}/collections/{collection}/dataStores/{dataStore} projects/{project}/locations/{location}/dataStores/{dataStore}</rdfs:comment>
    <rdfs:domain rdf:resource="http://example.org/onto/class/google_dialogflow_cx_tool"/>
    <rdfs:range rdf:resource="http://www.w3.org/2001/XMLSchema#string"/>
  </owl:DatatypeProperty>
  <owl:DatatypeProperty rdf:about="http://example.org/onto/prop/google_dialogflow_cx_tool_data_store_type">
    <rdfs:label>data_store_type</rdfs:label>
    <rdfs:comment>The type of the connected data store.
See [DataStoreType](https://cloud.google.com/dialogflow/cx/docs/reference/rest/v3/DataStoreConnection#datastoretype) for valid values.</rdfs:comment>
    <rdfs:domain rdf:resource="http://example.org/onto/class/google_dialogflow_cx_tool"/>
    <rdfs:range rdf:resource="http://www.w3.org/2001/XMLSchema#string"/>
  </owl:DatatypeProperty>
  <owl:DatatypeProperty rdf:about="http://example.org/onto/prop/google_dialogflow_cx_tool_document_processing_mode">
    <rdfs:label>document_processing_mode</rdfs:label>
    <rdfs:comment>The document processing mode for the data store connection. Should only be set for PUBLIC_WEB and UNSTRUCTURED data stores. If not set it is considered as DOCUMENTS, as this is the legacy mode.
See [DocumentProcessingMode](https://cloud.google.com/dialogflow/cx/docs/reference/rest/v3/DataStoreConnection#documentprocessingmode) for valid values.</rdfs:comment>
    <rdfs:domain rdf:resource="http://example.org/onto/class/google_dialogflow_cx_tool"/>
    <rdfs:range rdf:resource="http://www.w3.org/2001/XMLSchema#string"/>
  </owl:DatatypeProperty>
  <owl:DatatypeProperty rdf:about="http://example.org/onto/prop/google_dialogflow_cx_tool_input_schema">
    <rdfs:label>input_schema</rdfs:label>
    <rdfs:comment>Optional. The JSON schema is encapsulated in a [google.protobuf.Struct](https://protobuf.dev/reference/protobuf/google.protobuf/#struct) to describe the input of the function.
This input is a JSON object that contains the function's parameters as properties of the object</rdfs:comment>
    <rdfs:domain rdf:resource="http://example.org/onto/class/google_dialogflow_cx_tool"/>
    <rdfs:range rdf:resource="http://www.w3.org/2001/XMLSchema#string"/>
  </owl:DatatypeProperty>
  <owl:DatatypeProperty rdf:about="http://example.org/onto/prop/google_dialogflow_cx_tool_output_schema">
    <rdfs:label>output_schema</rdfs:label>
    <rdfs:comment>Optional. The JSON schema is encapsulated in a [google.protobuf.Struct](https://protobuf.dev/reference/protobuf/google.protobuf/#struct) to describe the output of the function.
This output is a JSON object that contains the function's parameters as properties of the object</rdfs:comment>
    <rdfs:domain rdf:resource="http://example.org/onto/class/google_dialogflow_cx_tool"/>
    <rdfs:range rdf:resource="http://www.w3.org/2001/XMLSchema#string"/>
  </owl:DatatypeProperty>
  <owl:DatatypeProperty rdf:about="http://example.org/onto/prop/google_dialogflow_cx_tool_text_schema">
    <rdfs:label>text_schema</rdfs:label>
    <rdfs:comment>The OpenAPI schema specified as a text.
This field is part of a union field 'schema': only one of 'textSchema' may be set.</rdfs:comment>
    <rdfs:domain rdf:resource="http://example.org/onto/class/google_dialogflow_cx_tool"/>
    <rdfs:range rdf:resource="http://www.w3.org/2001/XMLSchema#string"/>
  </owl:DatatypeProperty>
  <owl:DatatypeProperty rdf:about="http://example.org/onto/prop/google_dialogflow_cx_tool_api_key">
    <rdfs:label>api_key</rdfs:label>
    <rdfs:comment>Optional. The API key. If the 'secretVersionForApiKey'' field is set, this field will be ignored.</rdfs:comment>
    <rdfs:domain rdf:resource="http://example.org/onto/class/google_dialogflow_cx_tool"/>
    <rdfs:range rdf:resource="http://www.w3.org/2001/XMLSchema#string"/>
  </owl:DatatypeProperty>
  <owl:DatatypeProperty rdf:about="http://example.org/onto/prop/google_dialogflow_cx_tool_key_name">
    <rdfs:label>key_name</rdfs:label>
    <rdfs:comment>The parameter name or the header name of the API key.
E.g., If the API request is "https://example.com/act?X-Api-Key=", "X-Api-Key" would be the parameter name.</rdfs:comment>
    <rdfs:domain rdf:resource="http://example.org/onto/class/google_dialogflow_cx_tool"/>
    <rdfs:range rdf:resource="http://www.w3.org/2001/XMLSchema#string"/>
  </owl:DatatypeProperty>
  <owl:DatatypeProperty rdf:about="http://example.org/onto/prop/google_dialogflow_cx_tool_request_location">
    <rdfs:label>request_location</rdfs:label>
    <rdfs:comment>Key location in the request.
See [RequestLocation](https://cloud.google.com/dialogflow/cx/docs/reference/rest/v3/projects.locations.agents.tools#requestlocation) for valid values.</rdfs:comment>
    <rdfs:domain rdf:resource="http://example.org/onto/class/google_dialogflow_cx_tool"/>
    <rdfs:range rdf:resource="http://www.w3.org/2001/XMLSchema#string"/>
  </owl:DatatypeProperty>
  <owl:DatatypeProperty rdf:about="http://example.org/onto/prop/google_dialogflow_cx_tool_secret_version_for_api_key">
    <rdfs:label>secret_version_for_api_key</rdfs:label>
    <rdfs:comment>Optional. The name of the SecretManager secret version resource storing the API key.
If this field is set, the apiKey field will be ignored.
Format: projects/{project}/secrets/{secret}/versions/{version}</rdfs:comment>
    <rdfs:domain rdf:resource="http://example.org/onto/class/google_dialogflow_cx_tool"/>
    <rdfs:range rdf:resource="http://www.w3.org/2001/XMLSchema#string"/>
  </owl:DatatypeProperty>
  <owl:DatatypeProperty rdf:about="http://example.org/onto/prop/google_dialogflow_cx_tool_secret_version_for_token">
    <rdfs:label>secret_version_for_token</rdfs:label>
    <rdfs:comment>Optional. The name of the SecretManager secret version resource storing the Bearer token. If this field is set, the 'token' field will be ignored.
Format: projects/{project}/secrets/{secret}/versions/{version}</rdfs:comment>
    <rdfs:domain rdf:resource="http://example.org/onto/class/google_dialogflow_cx_tool"/>
    <rdfs:range rdf:resource="http://www.w3.org/2001/XMLSchema#string"/>
  </owl:DatatypeProperty>
  <owl:DatatypeProperty rdf:about="http://example.org/onto/prop/google_dialogflow_cx_tool_token">
    <rdfs:label>token</rdfs:label>
    <rdfs:comment>Optional. The text token appended to the text Bearer to the request Authorization header.
[Session parameters reference](https://cloud.google.com/dialogflow/cx/docs/concept/parameter#session-ref) can be used to pass the token dynamically, e.g. '$session.params.parameter-id'.</rdfs:comment>
    <rdfs:domain rdf:resource="http://example.org/onto/class/google_dialogflow_cx_tool"/>
    <rdfs:range rdf:resource="http://www.w3.org/2001/XMLSchema#string"/>
  </owl:DatatypeProperty>
  <owl:DatatypeProperty rdf:about="http://example.org/onto/prop/google_dialogflow_cx_tool_client_id">
    <rdfs:label>client_id</rdfs:label>
    <rdfs:comment>The client ID from the OAuth provider.</rdfs:comment>
    <rdfs:domain rdf:resource="http://example.org/onto/class/google_dialogflow_cx_tool"/>
    <rdfs:range rdf:resource="http://www.w3.org/2001/XMLSchema#string"/>
  </owl:DatatypeProperty>
  <owl:DatatypeProperty rdf:about="http://example.org/onto/prop/google_dialogflow_cx_tool_client_secret">
    <rdfs:label>client_secret</rdfs:label>
    <rdfs:comment>Optional. The client secret from the OAuth provider. If the 'secretVersionForClientSecret' field is set, this field will be ignored.</rdfs:comment>
    <rdfs:domain rdf:resource="http://example.org/onto/class/google_dialogflow_cx_tool"/>
    <rdfs:range rdf:resource="http://www.w3.org/2001/XMLSchema#string"/>
  </owl:DatatypeProperty>
  <owl:DatatypeProperty rdf:about="http://example.org/onto/prop/google_dialogflow_cx_tool_oauth_grant_type">
    <rdfs:label>oauth_grant_type</rdfs:label>
    <rdfs:comment>OAuth grant types.
See [OauthGrantType](https://cloud.google.com/dialogflow/cx/docs/reference/rest/v3/projects.locations.agents.tools#oauthgranttype) for valid values</rdfs:comment>
    <rdfs:domain rdf:resource="http://example.org/onto/class/google_dialogflow_cx_tool"/>
    <rdfs:range rdf:resource="http://www.w3.org/2001/XMLSchema#string"/>
  </owl:DatatypeProperty>
  <owl:DatatypeProperty rdf:about="http://example.org/onto/prop/google_dialogflow_cx_tool_scopes">
    <rdfs:label>scopes</rdfs:label>
    <rdfs:comment>Optional. The OAuth scopes to grant.</rdfs:comment>
    <rdfs:domain rdf:resource="http://example.org/onto/class/google_dialogflow_cx_tool"/>
    <rdfs:range rdf:resource="http://www.w3.org/2001/XMLSchema#string"/>
  </owl:DatatypeProperty>
  <owl:DatatypeProperty rdf:about="http://example.org/onto/prop/google_dialogflow_cx_tool_secret_version_for_client_secret">
    <rdfs:label>secret_version_for_client_secret</rdfs:label>
    <rdfs:comment>Optional. The name of the SecretManager secret version resource storing the client secret.
If this field is set, the clientSecret field will be ignored.
Format: projects/{project}/secrets/{secret}/versions/{version}</rdfs:comment>
    <rdfs:domain rdf:resource="http://example.org/onto/class/google_dialogflow_cx_tool"/>
    <rdfs:range rdf:resource="http://www.w3.org/2001/XMLSchema#string"/>
  </owl:DatatypeProperty>
  <owl:DatatypeProperty rdf:about="http://example.org/onto/prop/google_dialogflow_cx_tool_token_endpoint">
    <rdfs:label>token_endpoint</rdfs:label>
    <rdfs:comment>The token endpoint in the OAuth provider to exchange for an access token.</rdfs:comment>
    <rdfs:domain rdf:resource="http://example.org/onto/class/google_dialogflow_cx_tool"/>
    <rdfs:range rdf:resource="http://www.w3.org/2001/XMLSchema#string"/>
  </owl:DatatypeProperty>
  <owl:DatatypeProperty rdf:about="http://example.org/onto/prop/google_dialogflow_cx_tool_service_agent_auth">
    <rdfs:label>service_agent_auth</rdfs:label>
    <rdfs:comment>Optional. Indicate the auth token type generated from the Diglogflow service agent.
The generated token is sent in the Authorization header.
See [ServiceAgentAuth](https://cloud.google.com/dialogflow/cx/docs/reference/rest/v3/projects.locations.agents.tools#serviceagentauth) for valid values.</rdfs:comment>
    <rdfs:domain rdf:resource="http://example.org/onto/class/google_dialogflow_cx_tool"/>
    <rdfs:range rdf:resource="http://www.w3.org/2001/XMLSchema#string"/>
  </owl:DatatypeProperty>
  <owl:DatatypeProperty rdf:about="http://example.org/onto/prop/google_dialogflow_cx_tool_service">
    <rdfs:label>service</rdfs:label>
    <rdfs:comment>The name of [Service Directory](https://cloud.google.com/service-directory/docs) service.
Format: projects/<ProjectID>/locations/<LocationID>/namespaces/<NamespaceID>/services/<ServiceID>. LocationID of the service directory must be the same as the location of the agent.</rdfs:comment>
    <rdfs:domain rdf:resource="http://example.org/onto/class/google_dialogflow_cx_tool"/>
    <rdfs:range rdf:resource="http://www.w3.org/2001/XMLSchema#string"/>
  </owl:DatatypeProperty>
  <owl:DatatypeProperty rdf:about="http://example.org/onto/prop/google_dialogflow_cx_tool_cert">
    <rdfs:label>cert</rdfs:label>
    <rdfs:comment>The allowed custom CA certificates (in DER format) for HTTPS verification. This overrides the default SSL trust store.
If this is empty or unspecified, Dialogflow will use Google's default trust store to verify certificates.
N.B. Make sure the HTTPS server certificates are signed with "subject alt name".
For instance a certificate can be self-signed using the following command:
'''
  openssl x509 -req -days 200 -in example.com.csr \
    -signkey example.com.key \
    -out example.com.crt \
    -extfile <(printf "\nsubjectAltName='DNS:www.example.com'")
'''
A base64-encoded string.</rdfs:comment>
    <rdfs:domain rdf:resource="http://example.org/onto/class/google_dialogflow_cx_tool"/>
    <rdfs:range rdf:resource="http://www.w3.org/2001/XMLSchema#string"/>
  </owl:DatatypeProperty>
  <owl:DatatypeProperty rdf:about="http://example.org/onto/prop/google_dialogflow_cx_tool_display_name">
    <rdfs:label>display_name</rdfs:label>
    <rdfs:comment>The name of the allowed custom CA certificates. This can be used to disambiguate the custom CA certificates.</rdfs:comment>
    <rdfs:domain rdf:resource="http://example.org/onto/class/google_dialogflow_cx_tool"/>
    <rdfs:range rdf:resource="http://www.w3.org/2001/XMLSchema#string"/>
  </owl:DatatypeProperty>
  <owl:DatatypeProperty rdf:about="http://example.org/onto/prop/google_dialogflow_cx_tool_create">
    <rdfs:label>create</rdfs:label>
    <rdfs:domain rdf:resource="http://example.org/onto/class/google_dialogflow_cx_tool"/>
    <rdfs:range rdf:resource="http://www.w3.org/2001/XMLSchema#string"/>
  </owl:DatatypeProperty>
  <owl:DatatypeProperty rdf:about="http://example.org/onto/prop/google_dialogflow_cx_tool_delete">
    <rdfs:label>delete</rdfs:label>
    <rdfs:domain rdf:resource="http://example.org/onto/class/google_dialogflow_cx_tool"/>
    <rdfs:range rdf:resource="http://www.w3.org/2001/XMLSchema#string"/>
  </owl:DatatypeProperty>
  <owl:DatatypeProperty rdf:about="http://example.org/onto/prop/google_dialogflow_cx_tool_update">
    <rdfs:label>update</rdfs:label>
    <rdfs:domain rdf:resource="http://example.org/onto/class/google_dialogflow_cx_tool"/>
    <rdfs:range rdf:resource="http://www.w3.org/2001/XMLSchema#string"/>
  </owl:DatatypeProperty>
</rdf:RDF>
