<?xml version="1.0" encoding="UTF-8"?>
<rdf:RDF
  xmlns:rdf="http://www.w3.org/1999/02/22-rdf-syntax-ns#"
  xmlns:rdfs="http://www.w3.org/2000/01/rdf-schema#"
  xmlns:owl="http://www.w3.org/2002/07/owl#"
  xmlns:xsd="http://www.w3.org/2001/XMLSchema#"
  xml:base="http://example.org/onto/">
  <owl:Class rdf:about="http://example.org/onto/class/google_dataproc_metastore_service">
    <rdfs:label>google_dataproc_metastore_service</rdfs:label>
    <rdfs:comment>#
#     ***     AUTO GENERATED CODE    ***    Type: MMv1     ***
#
# ----------------------------------------------------------------------------
#
#     This code is generated by Magic Modules using the following:
#
#     Configuration: https:#github.com/GoogleCloudPlatform/magic-modules/tree/main/mmv1/products/metastore/Service.yaml
#     Template:      https:#github.com/GoogleCloudPlatform/magic-modules/tree/main/mmv1/templates/terraform/resource.html.markdown.tmpl
#
#     DO NOT EDIT this file directly. Any changes made to this file will be
#     overwritten during the next generation cycle.
#
# ----------------------------------------------------------------------------
subcategory: "Dataproc Metastore"
description: |-
  A managed metastore service that serves metadata queries.
---</rdfs:comment>
  </owl:Class>
  <owl:DatatypeProperty rdf:about="http://example.org/onto/prop/google_dataproc_metastore_service_artifact_gcs_uri">
    <rdfs:label>artifact_gcs_uri</rdfs:label>
    <rdfs:comment>A Cloud Storage URI (starting with gs://) that specifies where artifacts related to the metastore service are stored.</rdfs:comment>
    <rdfs:domain rdf:resource="http://example.org/onto/class/google_dataproc_metastore_service"/>
    <rdfs:range rdf:resource="http://www.w3.org/2001/XMLSchema#string"/>
  </owl:DatatypeProperty>
  <owl:DatatypeProperty rdf:about="http://example.org/onto/prop/google_dataproc_metastore_service_create_time">
    <rdfs:label>create_time</rdfs:label>
    <rdfs:comment>Output only. The time when the metastore service was created.</rdfs:comment>
    <rdfs:domain rdf:resource="http://example.org/onto/class/google_dataproc_metastore_service"/>
    <rdfs:range rdf:resource="http://www.w3.org/2001/XMLSchema#string"/>
  </owl:DatatypeProperty>
  <owl:DatatypeProperty rdf:about="http://example.org/onto/prop/google_dataproc_metastore_service_database_type">
    <rdfs:label>database_type</rdfs:label>
    <rdfs:comment>The database type that the Metastore service stores its data. Default value: "MYSQL" Possible values: ["MYSQL", "SPANNER"]</rdfs:comment>
    <rdfs:domain rdf:resource="http://example.org/onto/class/google_dataproc_metastore_service"/>
    <rdfs:range rdf:resource="http://www.w3.org/2001/XMLSchema#string"/>
  </owl:DatatypeProperty>
  <owl:DatatypeProperty rdf:about="http://example.org/onto/prop/google_dataproc_metastore_service_deletion_protection">
    <rdfs:label>deletion_protection</rdfs:label>
    <rdfs:comment>Indicates if the dataproc metastore should be protected against accidental deletions.</rdfs:comment>
    <rdfs:domain rdf:resource="http://example.org/onto/class/google_dataproc_metastore_service"/>
    <rdfs:range rdf:resource="http://www.w3.org/2001/XMLSchema#string"/>
  </owl:DatatypeProperty>
  <owl:DatatypeProperty rdf:about="http://example.org/onto/prop/google_dataproc_metastore_service_effective_labels">
    <rdfs:label>effective_labels</rdfs:label>
    <rdfs:comment>All of labels (key/value pairs) present on the resource in GCP, including the labels configured through Terraform, other clients and services.</rdfs:comment>
    <rdfs:domain rdf:resource="http://example.org/onto/class/google_dataproc_metastore_service"/>
    <rdfs:range rdf:resource="http://www.w3.org/2001/XMLSchema#string"/>
  </owl:DatatypeProperty>
  <owl:DatatypeProperty rdf:about="http://example.org/onto/prop/google_dataproc_metastore_service_endpoint_uri">
    <rdfs:label>endpoint_uri</rdfs:label>
    <rdfs:comment>The URI of the endpoint used to access the metastore service.</rdfs:comment>
    <rdfs:domain rdf:resource="http://example.org/onto/class/google_dataproc_metastore_service"/>
    <rdfs:range rdf:resource="http://www.w3.org/2001/XMLSchema#string"/>
  </owl:DatatypeProperty>
  <owl:DatatypeProperty rdf:about="http://example.org/onto/prop/google_dataproc_metastore_service_id">
    <rdfs:label>id</rdfs:label>
    <rdfs:domain rdf:resource="http://example.org/onto/class/google_dataproc_metastore_service"/>
    <rdfs:range rdf:resource="http://www.w3.org/2001/XMLSchema#string"/>
  </owl:DatatypeProperty>
  <owl:DatatypeProperty rdf:about="http://example.org/onto/prop/google_dataproc_metastore_service_labels">
    <rdfs:label>labels</rdfs:label>
    <rdfs:comment>User-defined labels for the metastore service.

**Note**: This field is non-authoritative, and will only manage the labels present in your configuration.
Please refer to the field 'effective_labels' for all of the labels present on the resource.</rdfs:comment>
    <rdfs:domain rdf:resource="http://example.org/onto/class/google_dataproc_metastore_service"/>
    <rdfs:range rdf:resource="http://www.w3.org/2001/XMLSchema#string"/>
  </owl:DatatypeProperty>
  <owl:DatatypeProperty rdf:about="http://example.org/onto/prop/google_dataproc_metastore_service_location">
    <rdfs:label>location</rdfs:label>
    <rdfs:comment>The location where the metastore service should reside.
The default value is 'global'.</rdfs:comment>
    <rdfs:domain rdf:resource="http://example.org/onto/class/google_dataproc_metastore_service"/>
    <rdfs:range rdf:resource="http://www.w3.org/2001/XMLSchema#string"/>
  </owl:DatatypeProperty>
  <owl:DatatypeProperty rdf:about="http://example.org/onto/prop/google_dataproc_metastore_service_name">
    <rdfs:label>name</rdfs:label>
    <rdfs:comment>The relative resource name of the metastore service.</rdfs:comment>
    <rdfs:domain rdf:resource="http://example.org/onto/class/google_dataproc_metastore_service"/>
    <rdfs:range rdf:resource="http://www.w3.org/2001/XMLSchema#string"/>
  </owl:DatatypeProperty>
  <owl:DatatypeProperty rdf:about="http://example.org/onto/prop/google_dataproc_metastore_service_network">
    <rdfs:label>network</rdfs:label>
    <rdfs:comment>The relative resource name of the VPC network on which the instance can be accessed. It is specified in the following form:

"projects/{projectNumber}/global/networks/{network_id}".</rdfs:comment>
    <rdfs:domain rdf:resource="http://example.org/onto/class/google_dataproc_metastore_service"/>
    <rdfs:range rdf:resource="http://www.w3.org/2001/XMLSchema#string"/>
  </owl:DatatypeProperty>
  <owl:DatatypeProperty rdf:about="http://example.org/onto/prop/google_dataproc_metastore_service_port">
    <rdfs:label>port</rdfs:label>
    <rdfs:comment>The TCP port at which the metastore service is reached. Default: 9083.</rdfs:comment>
    <rdfs:domain rdf:resource="http://example.org/onto/class/google_dataproc_metastore_service"/>
    <rdfs:range rdf:resource="http://www.w3.org/2001/XMLSchema#string"/>
  </owl:DatatypeProperty>
  <owl:DatatypeProperty rdf:about="http://example.org/onto/prop/google_dataproc_metastore_service_project">
    <rdfs:label>project</rdfs:label>
    <rdfs:domain rdf:resource="http://example.org/onto/class/google_dataproc_metastore_service"/>
    <rdfs:range rdf:resource="http://www.w3.org/2001/XMLSchema#string"/>
  </owl:DatatypeProperty>
  <owl:DatatypeProperty rdf:about="http://example.org/onto/prop/google_dataproc_metastore_service_release_channel">
    <rdfs:label>release_channel</rdfs:label>
    <rdfs:comment>The release channel of the service. If unspecified, defaults to 'STABLE'. Default value: "STABLE" Possible values: ["CANARY", "STABLE"]</rdfs:comment>
    <rdfs:domain rdf:resource="http://example.org/onto/class/google_dataproc_metastore_service"/>
    <rdfs:range rdf:resource="http://www.w3.org/2001/XMLSchema#string"/>
  </owl:DatatypeProperty>
  <owl:DatatypeProperty rdf:about="http://example.org/onto/prop/google_dataproc_metastore_service_service_id">
    <rdfs:label>service_id</rdfs:label>
    <rdfs:comment>The ID of the metastore service. The id must contain only letters (a-z, A-Z), numbers (0-9), underscores (_),
and hyphens (-). Cannot begin or end with underscore or hyphen. Must consist of between
3 and 63 characters.</rdfs:comment>
    <rdfs:domain rdf:resource="http://example.org/onto/class/google_dataproc_metastore_service"/>
    <rdfs:range rdf:resource="http://www.w3.org/2001/XMLSchema#string"/>
  </owl:DatatypeProperty>
  <owl:DatatypeProperty rdf:about="http://example.org/onto/prop/google_dataproc_metastore_service_state">
    <rdfs:label>state</rdfs:label>
    <rdfs:comment>The current state of the metastore service.</rdfs:comment>
    <rdfs:domain rdf:resource="http://example.org/onto/class/google_dataproc_metastore_service"/>
    <rdfs:range rdf:resource="http://www.w3.org/2001/XMLSchema#string"/>
  </owl:DatatypeProperty>
  <owl:DatatypeProperty rdf:about="http://example.org/onto/prop/google_dataproc_metastore_service_state_message">
    <rdfs:label>state_message</rdfs:label>
    <rdfs:comment>Additional information about the current state of the metastore service, if available.</rdfs:comment>
    <rdfs:domain rdf:resource="http://example.org/onto/class/google_dataproc_metastore_service"/>
    <rdfs:range rdf:resource="http://www.w3.org/2001/XMLSchema#string"/>
  </owl:DatatypeProperty>
  <owl:DatatypeProperty rdf:about="http://example.org/onto/prop/google_dataproc_metastore_service_tags">
    <rdfs:label>tags</rdfs:label>
    <rdfs:comment>A map of resource manager tags.
Resource manager tag keys and values have the same definition as resource manager tags.
Keys must be in the format tagKeys/{tag_key_id}, and values are in the format tagValues/{tag_value_id}.</rdfs:comment>
    <rdfs:domain rdf:resource="http://example.org/onto/class/google_dataproc_metastore_service"/>
    <rdfs:range rdf:resource="http://www.w3.org/2001/XMLSchema#string"/>
  </owl:DatatypeProperty>
  <owl:DatatypeProperty rdf:about="http://example.org/onto/prop/google_dataproc_metastore_service_terraform_labels">
    <rdfs:label>terraform_labels</rdfs:label>
    <rdfs:comment>The combination of labels configured directly on the resource
 and default labels configured on the provider.</rdfs:comment>
    <rdfs:domain rdf:resource="http://example.org/onto/class/google_dataproc_metastore_service"/>
    <rdfs:range rdf:resource="http://www.w3.org/2001/XMLSchema#string"/>
  </owl:DatatypeProperty>
  <owl:DatatypeProperty rdf:about="http://example.org/onto/prop/google_dataproc_metastore_service_tier">
    <rdfs:label>tier</rdfs:label>
    <rdfs:comment>The tier of the service. Possible values: ["DEVELOPER", "ENTERPRISE"]</rdfs:comment>
    <rdfs:domain rdf:resource="http://example.org/onto/class/google_dataproc_metastore_service"/>
    <rdfs:range rdf:resource="http://www.w3.org/2001/XMLSchema#string"/>
  </owl:DatatypeProperty>
  <owl:DatatypeProperty rdf:about="http://example.org/onto/prop/google_dataproc_metastore_service_uid">
    <rdfs:label>uid</rdfs:label>
    <rdfs:comment>The globally unique resource identifier of the metastore service.</rdfs:comment>
    <rdfs:domain rdf:resource="http://example.org/onto/class/google_dataproc_metastore_service"/>
    <rdfs:range rdf:resource="http://www.w3.org/2001/XMLSchema#string"/>
  </owl:DatatypeProperty>
  <owl:DatatypeProperty rdf:about="http://example.org/onto/prop/google_dataproc_metastore_service_update_time">
    <rdfs:label>update_time</rdfs:label>
    <rdfs:comment>Output only. The time when the metastore service was last updated.</rdfs:comment>
    <rdfs:domain rdf:resource="http://example.org/onto/class/google_dataproc_metastore_service"/>
    <rdfs:range rdf:resource="http://www.w3.org/2001/XMLSchema#string"/>
  </owl:DatatypeProperty>
  <owl:DatatypeProperty rdf:about="http://example.org/onto/prop/google_dataproc_metastore_service_kms_key">
    <rdfs:label>kms_key</rdfs:label>
    <rdfs:comment>The fully qualified customer provided Cloud KMS key name to use for customer data encryption.
Use the following format: 'projects/([^/]+)/locations/([^/]+)/keyRings/([^/]+)/cryptoKeys/([^/]+)'</rdfs:comment>
    <rdfs:domain rdf:resource="http://example.org/onto/class/google_dataproc_metastore_service"/>
    <rdfs:range rdf:resource="http://www.w3.org/2001/XMLSchema#string"/>
  </owl:DatatypeProperty>
  <owl:DatatypeProperty rdf:about="http://example.org/onto/prop/google_dataproc_metastore_service_config_overrides">
    <rdfs:label>config_overrides</rdfs:label>
    <rdfs:comment>A mapping of Hive metastore configuration key-value pairs to apply to the Hive metastore (configured in hive-site.xml).
The mappings override system defaults (some keys cannot be overridden)</rdfs:comment>
    <rdfs:domain rdf:resource="http://example.org/onto/class/google_dataproc_metastore_service"/>
    <rdfs:range rdf:resource="http://www.w3.org/2001/XMLSchema#string"/>
  </owl:DatatypeProperty>
  <owl:DatatypeProperty rdf:about="http://example.org/onto/prop/google_dataproc_metastore_service_endpoint_protocol">
    <rdfs:label>endpoint_protocol</rdfs:label>
    <rdfs:comment>The protocol to use for the metastore service endpoint. If unspecified, defaults to 'THRIFT'. Default value: "THRIFT" Possible values: ["THRIFT", "GRPC"]</rdfs:comment>
    <rdfs:domain rdf:resource="http://example.org/onto/class/google_dataproc_metastore_service"/>
    <rdfs:range rdf:resource="http://www.w3.org/2001/XMLSchema#string"/>
  </owl:DatatypeProperty>
  <owl:DatatypeProperty rdf:about="http://example.org/onto/prop/google_dataproc_metastore_service_version">
    <rdfs:label>version</rdfs:label>
    <rdfs:comment>The Hive metastore schema version.</rdfs:comment>
    <rdfs:domain rdf:resource="http://example.org/onto/class/google_dataproc_metastore_service"/>
    <rdfs:range rdf:resource="http://www.w3.org/2001/XMLSchema#string"/>
  </owl:DatatypeProperty>
  <owl:DatatypeProperty rdf:about="http://example.org/onto/prop/google_dataproc_metastore_service_config_overrides">
    <rdfs:label>config_overrides</rdfs:label>
    <rdfs:comment>A mapping of Hive metastore configuration key-value pairs to apply to the auxiliary Hive metastore (configured in hive-site.xml) in addition to the primary version's overrides.
If keys are present in both the auxiliary version's overrides and the primary version's overrides, the value from the auxiliary version's overrides takes precedence.</rdfs:comment>
    <rdfs:domain rdf:resource="http://example.org/onto/class/google_dataproc_metastore_service"/>
    <rdfs:range rdf:resource="http://www.w3.org/2001/XMLSchema#string"/>
  </owl:DatatypeProperty>
  <owl:DatatypeProperty rdf:about="http://example.org/onto/prop/google_dataproc_metastore_service_key">
    <rdfs:label>key</rdfs:label>
    <rdfs:domain rdf:resource="http://example.org/onto/class/google_dataproc_metastore_service"/>
    <rdfs:range rdf:resource="http://www.w3.org/2001/XMLSchema#string"/>
  </owl:DatatypeProperty>
  <owl:DatatypeProperty rdf:about="http://example.org/onto/prop/google_dataproc_metastore_service_version">
    <rdfs:label>version</rdfs:label>
    <rdfs:comment>The Hive metastore version of the auxiliary service. It must be less than the primary Hive metastore service's version.</rdfs:comment>
    <rdfs:domain rdf:resource="http://example.org/onto/class/google_dataproc_metastore_service"/>
    <rdfs:range rdf:resource="http://www.w3.org/2001/XMLSchema#string"/>
  </owl:DatatypeProperty>
  <owl:DatatypeProperty rdf:about="http://example.org/onto/prop/google_dataproc_metastore_service_krb5_config_gcs_uri">
    <rdfs:label>krb5_config_gcs_uri</rdfs:label>
    <rdfs:comment>A Cloud Storage URI that specifies the path to a krb5.conf file. It is of the form gs://{bucket_name}/path/to/krb5.conf, although the file does not need to be named krb5.conf explicitly.</rdfs:comment>
    <rdfs:domain rdf:resource="http://example.org/onto/class/google_dataproc_metastore_service"/>
    <rdfs:range rdf:resource="http://www.w3.org/2001/XMLSchema#string"/>
  </owl:DatatypeProperty>
  <owl:DatatypeProperty rdf:about="http://example.org/onto/prop/google_dataproc_metastore_service_principal">
    <rdfs:label>principal</rdfs:label>
    <rdfs:comment>A Kerberos principal that exists in the both the keytab the KDC to authenticate as. A typical principal is of the form "primary/instance@REALM", but there is no exact format.</rdfs:comment>
    <rdfs:domain rdf:resource="http://example.org/onto/class/google_dataproc_metastore_service"/>
    <rdfs:range rdf:resource="http://www.w3.org/2001/XMLSchema#string"/>
  </owl:DatatypeProperty>
  <owl:DatatypeProperty rdf:about="http://example.org/onto/prop/google_dataproc_metastore_service_cloud_secret">
    <rdfs:label>cloud_secret</rdfs:label>
    <rdfs:comment>The relative resource name of a Secret Manager secret version, in the following form:

"projects/{projectNumber}/secrets/{secret_id}/versions/{version_id}".</rdfs:comment>
    <rdfs:domain rdf:resource="http://example.org/onto/class/google_dataproc_metastore_service"/>
    <rdfs:range rdf:resource="http://www.w3.org/2001/XMLSchema#string"/>
  </owl:DatatypeProperty>
  <owl:DatatypeProperty rdf:about="http://example.org/onto/prop/google_dataproc_metastore_service_day_of_week">
    <rdfs:label>day_of_week</rdfs:label>
    <rdfs:comment>The day of week, when the window starts. Possible values: ["MONDAY", "TUESDAY", "WEDNESDAY", "THURSDAY", "FRIDAY", "SATURDAY", "SUNDAY"]</rdfs:comment>
    <rdfs:domain rdf:resource="http://example.org/onto/class/google_dataproc_metastore_service"/>
    <rdfs:range rdf:resource="http://www.w3.org/2001/XMLSchema#string"/>
  </owl:DatatypeProperty>
  <owl:DatatypeProperty rdf:about="http://example.org/onto/prop/google_dataproc_metastore_service_hour_of_day">
    <rdfs:label>hour_of_day</rdfs:label>
    <rdfs:comment>The hour of day (0-23) when the window starts.</rdfs:comment>
    <rdfs:domain rdf:resource="http://example.org/onto/class/google_dataproc_metastore_service"/>
    <rdfs:range rdf:resource="http://www.w3.org/2001/XMLSchema#string"/>
  </owl:DatatypeProperty>
  <owl:DatatypeProperty rdf:about="http://example.org/onto/prop/google_dataproc_metastore_service_enabled">
    <rdfs:label>enabled</rdfs:label>
    <rdfs:comment>Defines whether the metastore metadata should be synced to Data Catalog. The default value is to disable syncing metastore metadata to Data Catalog.</rdfs:comment>
    <rdfs:domain rdf:resource="http://example.org/onto/class/google_dataproc_metastore_service"/>
    <rdfs:range rdf:resource="http://www.w3.org/2001/XMLSchema#string"/>
  </owl:DatatypeProperty>
  <owl:DatatypeProperty rdf:about="http://example.org/onto/prop/google_dataproc_metastore_service_endpoint_uri">
    <rdfs:label>endpoint_uri</rdfs:label>
    <rdfs:comment>The URI of the endpoint used to access the metastore service.</rdfs:comment>
    <rdfs:domain rdf:resource="http://example.org/onto/class/google_dataproc_metastore_service"/>
    <rdfs:range rdf:resource="http://www.w3.org/2001/XMLSchema#string"/>
  </owl:DatatypeProperty>
  <owl:DatatypeProperty rdf:about="http://example.org/onto/prop/google_dataproc_metastore_service_subnetwork">
    <rdfs:label>subnetwork</rdfs:label>
    <rdfs:comment>The subnetwork of the customer project from which an IP address is reserved and used as the Dataproc Metastore service's endpoint.
It is accessible to hosts in the subnet and to all hosts in a subnet in the same region and same network.
There must be at least one IP address available in the subnet's primary range. The subnet is specified in the following form:
'projects/{projectNumber}/regions/{region_id}/subnetworks/{subnetwork_id}</rdfs:comment>
    <rdfs:domain rdf:resource="http://example.org/onto/class/google_dataproc_metastore_service"/>
    <rdfs:range rdf:resource="http://www.w3.org/2001/XMLSchema#string"/>
  </owl:DatatypeProperty>
  <owl:DatatypeProperty rdf:about="http://example.org/onto/prop/google_dataproc_metastore_service_instance_size">
    <rdfs:label>instance_size</rdfs:label>
    <rdfs:comment>Metastore instance sizes. Possible values: ["EXTRA_SMALL", "SMALL", "MEDIUM", "LARGE", "EXTRA_LARGE"]</rdfs:comment>
    <rdfs:domain rdf:resource="http://example.org/onto/class/google_dataproc_metastore_service"/>
    <rdfs:range rdf:resource="http://www.w3.org/2001/XMLSchema#string"/>
  </owl:DatatypeProperty>
  <owl:DatatypeProperty rdf:about="http://example.org/onto/prop/google_dataproc_metastore_service_scaling_factor">
    <rdfs:label>scaling_factor</rdfs:label>
    <rdfs:comment>Scaling factor, in increments of 0.1 for values less than 1.0, and increments of 1.0 for values greater than 1.0.</rdfs:comment>
    <rdfs:domain rdf:resource="http://example.org/onto/class/google_dataproc_metastore_service"/>
    <rdfs:range rdf:resource="http://www.w3.org/2001/XMLSchema#string"/>
  </owl:DatatypeProperty>
  <owl:DatatypeProperty rdf:about="http://example.org/onto/prop/google_dataproc_metastore_service_autoscaling_enabled">
    <rdfs:label>autoscaling_enabled</rdfs:label>
    <rdfs:comment>Defines whether autoscaling is enabled. The default value is false.</rdfs:comment>
    <rdfs:domain rdf:resource="http://example.org/onto/class/google_dataproc_metastore_service"/>
    <rdfs:range rdf:resource="http://www.w3.org/2001/XMLSchema#string"/>
  </owl:DatatypeProperty>
  <owl:DatatypeProperty rdf:about="http://example.org/onto/prop/google_dataproc_metastore_service_autoscaling_factor">
    <rdfs:label>autoscaling_factor</rdfs:label>
    <rdfs:comment>Output only. The scaling factor of a service with autoscaling enabled.</rdfs:comment>
    <rdfs:domain rdf:resource="http://example.org/onto/class/google_dataproc_metastore_service"/>
    <rdfs:range rdf:resource="http://www.w3.org/2001/XMLSchema#string"/>
  </owl:DatatypeProperty>
  <owl:DatatypeProperty rdf:about="http://example.org/onto/prop/google_dataproc_metastore_service_max_scaling_factor">
    <rdfs:label>max_scaling_factor</rdfs:label>
    <rdfs:comment>The maximum scaling factor that the service will autoscale to. The default value is 6.0.</rdfs:comment>
    <rdfs:domain rdf:resource="http://example.org/onto/class/google_dataproc_metastore_service"/>
    <rdfs:range rdf:resource="http://www.w3.org/2001/XMLSchema#string"/>
  </owl:DatatypeProperty>
  <owl:DatatypeProperty rdf:about="http://example.org/onto/prop/google_dataproc_metastore_service_min_scaling_factor">
    <rdfs:label>min_scaling_factor</rdfs:label>
    <rdfs:comment>The minimum scaling factor that the service will autoscale to. The default value is 0.1.</rdfs:comment>
    <rdfs:domain rdf:resource="http://example.org/onto/class/google_dataproc_metastore_service"/>
    <rdfs:range rdf:resource="http://www.w3.org/2001/XMLSchema#string"/>
  </owl:DatatypeProperty>
  <owl:DatatypeProperty rdf:about="http://example.org/onto/prop/google_dataproc_metastore_service_backup_location">
    <rdfs:label>backup_location</rdfs:label>
    <rdfs:comment>A Cloud Storage URI of a folder, in the format gs://<bucket_name>/<path_inside_bucket>. A sub-folder <backup_folder> containing backup files will be stored below it.</rdfs:comment>
    <rdfs:domain rdf:resource="http://example.org/onto/class/google_dataproc_metastore_service"/>
    <rdfs:range rdf:resource="http://www.w3.org/2001/XMLSchema#string"/>
  </owl:DatatypeProperty>
  <owl:DatatypeProperty rdf:about="http://example.org/onto/prop/google_dataproc_metastore_service_cron_schedule">
    <rdfs:label>cron_schedule</rdfs:label>
    <rdfs:comment>The scheduled interval in Cron format, see https://en.wikipedia.org/wiki/Cron The default is empty: scheduled backup is not enabled. Must be specified to enable scheduled backups.</rdfs:comment>
    <rdfs:domain rdf:resource="http://example.org/onto/class/google_dataproc_metastore_service"/>
    <rdfs:range rdf:resource="http://www.w3.org/2001/XMLSchema#string"/>
  </owl:DatatypeProperty>
  <owl:DatatypeProperty rdf:about="http://example.org/onto/prop/google_dataproc_metastore_service_enabled">
    <rdfs:label>enabled</rdfs:label>
    <rdfs:comment>Defines whether the scheduled backup is enabled. The default value is false.</rdfs:comment>
    <rdfs:domain rdf:resource="http://example.org/onto/class/google_dataproc_metastore_service"/>
    <rdfs:range rdf:resource="http://www.w3.org/2001/XMLSchema#string"/>
  </owl:DatatypeProperty>
  <owl:DatatypeProperty rdf:about="http://example.org/onto/prop/google_dataproc_metastore_service_time_zone">
    <rdfs:label>time_zone</rdfs:label>
    <rdfs:comment>Specifies the time zone to be used when interpreting cronSchedule. Must be a time zone name from the time zone database (https://en.wikipedia.org/wiki/List_of_tz_database_time_zones), e.g. America/Los_Angeles or Africa/Abidjan. If left unspecified, the default is UTC.</rdfs:comment>
    <rdfs:domain rdf:resource="http://example.org/onto/class/google_dataproc_metastore_service"/>
    <rdfs:range rdf:resource="http://www.w3.org/2001/XMLSchema#string"/>
  </owl:DatatypeProperty>
  <owl:DatatypeProperty rdf:about="http://example.org/onto/prop/google_dataproc_metastore_service_log_format">
    <rdfs:label>log_format</rdfs:label>
    <rdfs:comment>The output format of the Dataproc Metastore service's logs. Default value: "JSON" Possible values: ["LEGACY", "JSON"]</rdfs:comment>
    <rdfs:domain rdf:resource="http://example.org/onto/class/google_dataproc_metastore_service"/>
    <rdfs:range rdf:resource="http://www.w3.org/2001/XMLSchema#string"/>
  </owl:DatatypeProperty>
  <owl:DatatypeProperty rdf:about="http://example.org/onto/prop/google_dataproc_metastore_service_create">
    <rdfs:label>create</rdfs:label>
    <rdfs:domain rdf:resource="http://example.org/onto/class/google_dataproc_metastore_service"/>
    <rdfs:range rdf:resource="http://www.w3.org/2001/XMLSchema#string"/>
  </owl:DatatypeProperty>
  <owl:DatatypeProperty rdf:about="http://example.org/onto/prop/google_dataproc_metastore_service_delete">
    <rdfs:label>delete</rdfs:label>
    <rdfs:domain rdf:resource="http://example.org/onto/class/google_dataproc_metastore_service"/>
    <rdfs:range rdf:resource="http://www.w3.org/2001/XMLSchema#string"/>
  </owl:DatatypeProperty>
  <owl:DatatypeProperty rdf:about="http://example.org/onto/prop/google_dataproc_metastore_service_update">
    <rdfs:label>update</rdfs:label>
    <rdfs:domain rdf:resource="http://example.org/onto/class/google_dataproc_metastore_service"/>
    <rdfs:range rdf:resource="http://www.w3.org/2001/XMLSchema#string"/>
  </owl:DatatypeProperty>
</rdf:RDF>
