<?xml version="1.0" encoding="UTF-8"?>
<rdf:RDF
  xmlns:rdf="http://www.w3.org/1999/02/22-rdf-syntax-ns#"
  xmlns:rdfs="http://www.w3.org/2000/01/rdf-schema#"
  xmlns:owl="http://www.w3.org/2002/07/owl#"
  xmlns:xsd="http://www.w3.org/2001/XMLSchema#"
  xml:base="http://example.org/onto/">
  <owl:Class rdf:about="http://example.org/onto/class/google_dataplex_datascan">
    <rdfs:label>google_dataplex_datascan</rdfs:label>
    <rdfs:comment>#
#     ***     AUTO GENERATED CODE    ***    Type: MMv1     ***
#
# ----------------------------------------------------------------------------
#
#     This code is generated by Magic Modules using the following:
#
#     Configuration: https:#github.com/GoogleCloudPlatform/magic-modules/tree/main/mmv1/products/dataplex/Datascan.yaml
#     Template:      https:#github.com/GoogleCloudPlatform/magic-modules/tree/main/mmv1/templates/terraform/resource.html.markdown.tmpl
#
#     DO NOT EDIT this file directly. Any changes made to this file will be
#     overwritten during the next generation cycle.
#
# ----------------------------------------------------------------------------
subcategory: "Dataplex"
description: |-
  Represents a user-visible job which provides the insights for the related data source.
---</rdfs:comment>
  </owl:Class>
  <owl:DatatypeProperty rdf:about="http://example.org/onto/prop/google_dataplex_datascan_create_time">
    <rdfs:label>create_time</rdfs:label>
    <rdfs:comment>The time when the scan was created.</rdfs:comment>
    <rdfs:domain rdf:resource="http://example.org/onto/class/google_dataplex_datascan"/>
    <rdfs:range rdf:resource="http://www.w3.org/2001/XMLSchema#string"/>
  </owl:DatatypeProperty>
  <owl:DatatypeProperty rdf:about="http://example.org/onto/prop/google_dataplex_datascan_data_scan_id">
    <rdfs:label>data_scan_id</rdfs:label>
    <rdfs:comment>DataScan identifier. Must contain only lowercase letters, numbers and hyphens. Must start with a letter. Must end with a number or a letter.</rdfs:comment>
    <rdfs:domain rdf:resource="http://example.org/onto/class/google_dataplex_datascan"/>
    <rdfs:range rdf:resource="http://www.w3.org/2001/XMLSchema#string"/>
  </owl:DatatypeProperty>
  <owl:DatatypeProperty rdf:about="http://example.org/onto/prop/google_dataplex_datascan_description">
    <rdfs:label>description</rdfs:label>
    <rdfs:comment>Description of the scan.</rdfs:comment>
    <rdfs:domain rdf:resource="http://example.org/onto/class/google_dataplex_datascan"/>
    <rdfs:range rdf:resource="http://www.w3.org/2001/XMLSchema#string"/>
  </owl:DatatypeProperty>
  <owl:DatatypeProperty rdf:about="http://example.org/onto/prop/google_dataplex_datascan_display_name">
    <rdfs:label>display_name</rdfs:label>
    <rdfs:comment>User friendly display name.</rdfs:comment>
    <rdfs:domain rdf:resource="http://example.org/onto/class/google_dataplex_datascan"/>
    <rdfs:range rdf:resource="http://www.w3.org/2001/XMLSchema#string"/>
  </owl:DatatypeProperty>
  <owl:DatatypeProperty rdf:about="http://example.org/onto/prop/google_dataplex_datascan_effective_labels">
    <rdfs:label>effective_labels</rdfs:label>
    <rdfs:comment>All of labels (key/value pairs) present on the resource in GCP, including the labels configured through Terraform, other clients and services.</rdfs:comment>
    <rdfs:domain rdf:resource="http://example.org/onto/class/google_dataplex_datascan"/>
    <rdfs:range rdf:resource="http://www.w3.org/2001/XMLSchema#string"/>
  </owl:DatatypeProperty>
  <owl:DatatypeProperty rdf:about="http://example.org/onto/prop/google_dataplex_datascan_execution_status">
    <rdfs:label>execution_status</rdfs:label>
    <rdfs:comment>Status of the data scan execution.</rdfs:comment>
    <rdfs:domain rdf:resource="http://example.org/onto/class/google_dataplex_datascan"/>
    <rdfs:range rdf:resource="http://www.w3.org/2001/XMLSchema#string"/>
  </owl:DatatypeProperty>
  <owl:DatatypeProperty rdf:about="http://example.org/onto/prop/google_dataplex_datascan_id">
    <rdfs:label>id</rdfs:label>
    <rdfs:domain rdf:resource="http://example.org/onto/class/google_dataplex_datascan"/>
    <rdfs:range rdf:resource="http://www.w3.org/2001/XMLSchema#string"/>
  </owl:DatatypeProperty>
  <owl:DatatypeProperty rdf:about="http://example.org/onto/prop/google_dataplex_datascan_labels">
    <rdfs:label>labels</rdfs:label>
    <rdfs:comment>User-defined labels for the scan. A list of key->value pairs.


**Note**: This field is non-authoritative, and will only manage the labels present in your configuration.
Please refer to the field 'effective_labels' for all of the labels present on the resource.</rdfs:comment>
    <rdfs:domain rdf:resource="http://example.org/onto/class/google_dataplex_datascan"/>
    <rdfs:range rdf:resource="http://www.w3.org/2001/XMLSchema#string"/>
  </owl:DatatypeProperty>
  <owl:DatatypeProperty rdf:about="http://example.org/onto/prop/google_dataplex_datascan_location">
    <rdfs:label>location</rdfs:label>
    <rdfs:comment>The location where the data scan should reside.</rdfs:comment>
    <rdfs:domain rdf:resource="http://example.org/onto/class/google_dataplex_datascan"/>
    <rdfs:range rdf:resource="http://www.w3.org/2001/XMLSchema#string"/>
  </owl:DatatypeProperty>
  <owl:DatatypeProperty rdf:about="http://example.org/onto/prop/google_dataplex_datascan_name">
    <rdfs:label>name</rdfs:label>
    <rdfs:comment>The relative resource name of the scan, of the form: projects/{project}/locations/{locationId}/dataScans/{datascan_id}, where project refers to a project_id or project_number and locationId refers to a GCP region.</rdfs:comment>
    <rdfs:domain rdf:resource="http://example.org/onto/class/google_dataplex_datascan"/>
    <rdfs:range rdf:resource="http://www.w3.org/2001/XMLSchema#string"/>
  </owl:DatatypeProperty>
  <owl:DatatypeProperty rdf:about="http://example.org/onto/prop/google_dataplex_datascan_project">
    <rdfs:label>project</rdfs:label>
    <rdfs:domain rdf:resource="http://example.org/onto/class/google_dataplex_datascan"/>
    <rdfs:range rdf:resource="http://www.w3.org/2001/XMLSchema#string"/>
  </owl:DatatypeProperty>
  <owl:DatatypeProperty rdf:about="http://example.org/onto/prop/google_dataplex_datascan_state">
    <rdfs:label>state</rdfs:label>
    <rdfs:comment>Current state of the DataScan.</rdfs:comment>
    <rdfs:domain rdf:resource="http://example.org/onto/class/google_dataplex_datascan"/>
    <rdfs:range rdf:resource="http://www.w3.org/2001/XMLSchema#string"/>
  </owl:DatatypeProperty>
  <owl:DatatypeProperty rdf:about="http://example.org/onto/prop/google_dataplex_datascan_terraform_labels">
    <rdfs:label>terraform_labels</rdfs:label>
    <rdfs:comment>The combination of labels configured directly on the resource
 and default labels configured on the provider.</rdfs:comment>
    <rdfs:domain rdf:resource="http://example.org/onto/class/google_dataplex_datascan"/>
    <rdfs:range rdf:resource="http://www.w3.org/2001/XMLSchema#string"/>
  </owl:DatatypeProperty>
  <owl:DatatypeProperty rdf:about="http://example.org/onto/prop/google_dataplex_datascan_type">
    <rdfs:label>type</rdfs:label>
    <rdfs:comment>The type of DataScan.</rdfs:comment>
    <rdfs:domain rdf:resource="http://example.org/onto/class/google_dataplex_datascan"/>
    <rdfs:range rdf:resource="http://www.w3.org/2001/XMLSchema#string"/>
  </owl:DatatypeProperty>
  <owl:DatatypeProperty rdf:about="http://example.org/onto/prop/google_dataplex_datascan_uid">
    <rdfs:label>uid</rdfs:label>
    <rdfs:comment>System generated globally unique ID for the scan. This ID will be different if the scan is deleted and re-created with the same name.</rdfs:comment>
    <rdfs:domain rdf:resource="http://example.org/onto/class/google_dataplex_datascan"/>
    <rdfs:range rdf:resource="http://www.w3.org/2001/XMLSchema#string"/>
  </owl:DatatypeProperty>
  <owl:DatatypeProperty rdf:about="http://example.org/onto/prop/google_dataplex_datascan_update_time">
    <rdfs:label>update_time</rdfs:label>
    <rdfs:comment>The time when the scan was last updated.</rdfs:comment>
    <rdfs:domain rdf:resource="http://example.org/onto/class/google_dataplex_datascan"/>
    <rdfs:range rdf:resource="http://www.w3.org/2001/XMLSchema#string"/>
  </owl:DatatypeProperty>
  <owl:DatatypeProperty rdf:about="http://example.org/onto/prop/google_dataplex_datascan_entity">
    <rdfs:label>entity</rdfs:label>
    <rdfs:comment>The Dataplex entity that represents the data source(e.g. BigQuery table) for Datascan.</rdfs:comment>
    <rdfs:domain rdf:resource="http://example.org/onto/class/google_dataplex_datascan"/>
    <rdfs:range rdf:resource="http://www.w3.org/2001/XMLSchema#string"/>
  </owl:DatatypeProperty>
  <owl:DatatypeProperty rdf:about="http://example.org/onto/prop/google_dataplex_datascan_resource">
    <rdfs:label>resource</rdfs:label>
    <rdfs:comment>The service-qualified full resource name of the cloud resource for a DataScan job to scan against. The field could be:
Cloud Storage bucket (//storage.googleapis.com/projects/PROJECT_ID/buckets/BUCKET_ID) for DataDiscoveryScan OR BigQuery table of type "TABLE" (/bigquery.googleapis.com/projects/PROJECT_ID/datasets/DATASET_ID/tables/TABLE_ID) for DataProfileScan/DataQualityScan.</rdfs:comment>
    <rdfs:domain rdf:resource="http://example.org/onto/class/google_dataplex_datascan"/>
    <rdfs:range rdf:resource="http://www.w3.org/2001/XMLSchema#string"/>
  </owl:DatatypeProperty>
  <owl:DatatypeProperty rdf:about="http://example.org/onto/prop/google_dataplex_datascan_connection">
    <rdfs:label>connection</rdfs:label>
    <rdfs:comment>The BigQuery connection used to create BigLake tables. Must be in the form 'projects/{projectId}/locations/{locationId}/connections/{connection_id}'.</rdfs:comment>
    <rdfs:domain rdf:resource="http://example.org/onto/class/google_dataplex_datascan"/>
    <rdfs:range rdf:resource="http://www.w3.org/2001/XMLSchema#string"/>
  </owl:DatatypeProperty>
  <owl:DatatypeProperty rdf:about="http://example.org/onto/prop/google_dataplex_datascan_location">
    <rdfs:label>location</rdfs:label>
    <rdfs:comment>The location of the BigQuery dataset to publish BigLake external or non-BigLake external tables to.</rdfs:comment>
    <rdfs:domain rdf:resource="http://example.org/onto/class/google_dataplex_datascan"/>
    <rdfs:range rdf:resource="http://www.w3.org/2001/XMLSchema#string"/>
  </owl:DatatypeProperty>
  <owl:DatatypeProperty rdf:about="http://example.org/onto/prop/google_dataplex_datascan_project">
    <rdfs:label>project</rdfs:label>
    <rdfs:comment>The project of the BigQuery dataset to publish BigLake external or non-BigLake external tables to. If not specified, the project of the Cloud Storage bucket will be used. The format is "projects/{project_id_or_number}".</rdfs:comment>
    <rdfs:domain rdf:resource="http://example.org/onto/class/google_dataplex_datascan"/>
    <rdfs:range rdf:resource="http://www.w3.org/2001/XMLSchema#string"/>
  </owl:DatatypeProperty>
  <owl:DatatypeProperty rdf:about="http://example.org/onto/prop/google_dataplex_datascan_table_type">
    <rdfs:label>table_type</rdfs:label>
    <rdfs:comment>Determines whether to publish discovered tables as BigLake external tables or non-BigLake external tables. Possible values: ["TABLE_TYPE_UNSPECIFIED", "EXTERNAL", "BIGLAKE"]</rdfs:comment>
    <rdfs:domain rdf:resource="http://example.org/onto/class/google_dataplex_datascan"/>
    <rdfs:range rdf:resource="http://www.w3.org/2001/XMLSchema#string"/>
  </owl:DatatypeProperty>
  <owl:DatatypeProperty rdf:about="http://example.org/onto/prop/google_dataplex_datascan_exclude_patterns">
    <rdfs:label>exclude_patterns</rdfs:label>
    <rdfs:comment>Defines the data to exclude during discovery. Provide a list of patterns that identify the data to exclude. For Cloud Storage bucket assets, these patterns are interpreted as glob patterns used to match object names. For BigQuery dataset assets, these patterns are interpreted as patterns to match table names.</rdfs:comment>
    <rdfs:domain rdf:resource="http://example.org/onto/class/google_dataplex_datascan"/>
    <rdfs:range rdf:resource="http://www.w3.org/2001/XMLSchema#string"/>
  </owl:DatatypeProperty>
  <owl:DatatypeProperty rdf:about="http://example.org/onto/prop/google_dataplex_datascan_include_patterns">
    <rdfs:label>include_patterns</rdfs:label>
    <rdfs:comment>Defines the data to include during discovery when only a subset of the data should be considered. Provide a list of patterns that identify the data to include. For Cloud Storage bucket assets, these patterns are interpreted as glob patterns used to match object names. For BigQuery dataset assets, these patterns are interpreted as patterns to match table names.</rdfs:comment>
    <rdfs:domain rdf:resource="http://example.org/onto/class/google_dataplex_datascan"/>
    <rdfs:range rdf:resource="http://www.w3.org/2001/XMLSchema#string"/>
  </owl:DatatypeProperty>
  <owl:DatatypeProperty rdf:about="http://example.org/onto/prop/google_dataplex_datascan_delimiter">
    <rdfs:label>delimiter</rdfs:label>
    <rdfs:comment>The delimiter that is used to separate values. The default is ',' (comma).</rdfs:comment>
    <rdfs:domain rdf:resource="http://example.org/onto/class/google_dataplex_datascan"/>
    <rdfs:range rdf:resource="http://www.w3.org/2001/XMLSchema#string"/>
  </owl:DatatypeProperty>
  <owl:DatatypeProperty rdf:about="http://example.org/onto/prop/google_dataplex_datascan_encoding">
    <rdfs:label>encoding</rdfs:label>
    <rdfs:comment>The character encoding of the data. The default is UTF-8.</rdfs:comment>
    <rdfs:domain rdf:resource="http://example.org/onto/class/google_dataplex_datascan"/>
    <rdfs:range rdf:resource="http://www.w3.org/2001/XMLSchema#string"/>
  </owl:DatatypeProperty>
  <owl:DatatypeProperty rdf:about="http://example.org/onto/prop/google_dataplex_datascan_header_rows">
    <rdfs:label>header_rows</rdfs:label>
    <rdfs:comment>The number of rows to interpret as header rows that should be skipped when reading data rows.</rdfs:comment>
    <rdfs:domain rdf:resource="http://example.org/onto/class/google_dataplex_datascan"/>
    <rdfs:range rdf:resource="http://www.w3.org/2001/XMLSchema#string"/>
  </owl:DatatypeProperty>
  <owl:DatatypeProperty rdf:about="http://example.org/onto/prop/google_dataplex_datascan_quote">
    <rdfs:label>quote</rdfs:label>
    <rdfs:comment>The character used to quote column values. Accepts '"' (double quotation mark) or ''' (single quotation mark). If unspecified, defaults to '"' (double quotation mark).</rdfs:comment>
    <rdfs:domain rdf:resource="http://example.org/onto/class/google_dataplex_datascan"/>
    <rdfs:range rdf:resource="http://www.w3.org/2001/XMLSchema#string"/>
  </owl:DatatypeProperty>
  <owl:DatatypeProperty rdf:about="http://example.org/onto/prop/google_dataplex_datascan_type_inference_disabled">
    <rdfs:label>type_inference_disabled</rdfs:label>
    <rdfs:comment>Whether to disable the inference of data types for CSV data. If true, all columns are registered as strings.</rdfs:comment>
    <rdfs:domain rdf:resource="http://example.org/onto/class/google_dataplex_datascan"/>
    <rdfs:range rdf:resource="http://www.w3.org/2001/XMLSchema#string"/>
  </owl:DatatypeProperty>
  <owl:DatatypeProperty rdf:about="http://example.org/onto/prop/google_dataplex_datascan_encoding">
    <rdfs:label>encoding</rdfs:label>
    <rdfs:comment>The character encoding of the data. The default is UTF-8.</rdfs:comment>
    <rdfs:domain rdf:resource="http://example.org/onto/class/google_dataplex_datascan"/>
    <rdfs:range rdf:resource="http://www.w3.org/2001/XMLSchema#string"/>
  </owl:DatatypeProperty>
  <owl:DatatypeProperty rdf:about="http://example.org/onto/prop/google_dataplex_datascan_type_inference_disabled">
    <rdfs:label>type_inference_disabled</rdfs:label>
    <rdfs:comment>Whether to disable the inference of data types for JSON data. If true, all columns are registered as their primitive types (strings, number, or boolean).</rdfs:comment>
    <rdfs:domain rdf:resource="http://example.org/onto/class/google_dataplex_datascan"/>
    <rdfs:range rdf:resource="http://www.w3.org/2001/XMLSchema#string"/>
  </owl:DatatypeProperty>
  <owl:DatatypeProperty rdf:about="http://example.org/onto/prop/google_dataplex_datascan_row_filter">
    <rdfs:label>row_filter</rdfs:label>
    <rdfs:comment>A filter applied to all rows in a single DataScan job. The filter needs to be a valid SQL expression for a WHERE clause in BigQuery standard SQL syntax. Example: col1 >= 0 AND col2 < 10</rdfs:comment>
    <rdfs:domain rdf:resource="http://example.org/onto/class/google_dataplex_datascan"/>
    <rdfs:range rdf:resource="http://www.w3.org/2001/XMLSchema#string"/>
  </owl:DatatypeProperty>
  <owl:DatatypeProperty rdf:about="http://example.org/onto/prop/google_dataplex_datascan_sampling_percent">
    <rdfs:label>sampling_percent</rdfs:label>
    <rdfs:comment>The percentage of the records to be selected from the dataset for DataScan.
Value can range between 0.0 and 100.0 with up to 3 significant decimal digits.
Sampling is not applied if 'sampling_percent' is not specified, 0 or 100.</rdfs:comment>
    <rdfs:domain rdf:resource="http://example.org/onto/class/google_dataplex_datascan"/>
    <rdfs:range rdf:resource="http://www.w3.org/2001/XMLSchema#string"/>
  </owl:DatatypeProperty>
  <owl:DatatypeProperty rdf:about="http://example.org/onto/prop/google_dataplex_datascan_field_names">
    <rdfs:label>field_names</rdfs:label>
    <rdfs:comment>Expected input is a list of fully qualified names of fields as in the schema.
Only top-level field names for nested fields are supported.
For instance, if 'x' is of nested field type, listing 'x' is supported but 'x.y.z' is not supported. Here 'y' and 'y.z' are nested fields of 'x'.</rdfs:comment>
    <rdfs:domain rdf:resource="http://example.org/onto/class/google_dataplex_datascan"/>
    <rdfs:range rdf:resource="http://www.w3.org/2001/XMLSchema#string"/>
  </owl:DatatypeProperty>
  <owl:DatatypeProperty rdf:about="http://example.org/onto/prop/google_dataplex_datascan_field_names">
    <rdfs:label>field_names</rdfs:label>
    <rdfs:comment>Expected input is a list of fully qualified names of fields as in the schema.
Only top-level field names for nested fields are supported.
For instance, if 'x' is of nested field type, listing 'x' is supported but 'x.y.z' is not supported. Here 'y' and 'y.z' are nested fields of 'x'.</rdfs:comment>
    <rdfs:domain rdf:resource="http://example.org/onto/class/google_dataplex_datascan"/>
    <rdfs:range rdf:resource="http://www.w3.org/2001/XMLSchema#string"/>
  </owl:DatatypeProperty>
  <owl:DatatypeProperty rdf:about="http://example.org/onto/prop/google_dataplex_datascan_results_table">
    <rdfs:label>results_table</rdfs:label>
    <rdfs:comment>The BigQuery table to export DataProfileScan results to.
Format://bigquery.googleapis.com/projects/PROJECT_ID/datasets/DATASET_ID/tables/TABLE_ID</rdfs:comment>
    <rdfs:domain rdf:resource="http://example.org/onto/class/google_dataplex_datascan"/>
    <rdfs:range rdf:resource="http://www.w3.org/2001/XMLSchema#string"/>
  </owl:DatatypeProperty>
  <owl:DatatypeProperty rdf:about="http://example.org/onto/prop/google_dataplex_datascan_catalog_publishing_enabled">
    <rdfs:label>catalog_publishing_enabled</rdfs:label>
    <rdfs:comment>If set, the latest DataScan job result will be published to Dataplex Catalog.</rdfs:comment>
    <rdfs:domain rdf:resource="http://example.org/onto/class/google_dataplex_datascan"/>
    <rdfs:range rdf:resource="http://www.w3.org/2001/XMLSchema#string"/>
  </owl:DatatypeProperty>
  <owl:DatatypeProperty rdf:about="http://example.org/onto/prop/google_dataplex_datascan_row_filter">
    <rdfs:label>row_filter</rdfs:label>
    <rdfs:comment>A filter applied to all rows in a single DataScan job. The filter needs to be a valid SQL expression for a WHERE clause in BigQuery standard SQL syntax. Example: col1 >= 0 AND col2 < 10</rdfs:comment>
    <rdfs:domain rdf:resource="http://example.org/onto/class/google_dataplex_datascan"/>
    <rdfs:range rdf:resource="http://www.w3.org/2001/XMLSchema#string"/>
  </owl:DatatypeProperty>
  <owl:DatatypeProperty rdf:about="http://example.org/onto/prop/google_dataplex_datascan_sampling_percent">
    <rdfs:label>sampling_percent</rdfs:label>
    <rdfs:comment>The percentage of the records to be selected from the dataset for DataScan.
Value can range between 0.0 and 100.0 with up to 3 significant decimal digits.
Sampling is not applied if 'sampling_percent' is not specified, 0 or 100.</rdfs:comment>
    <rdfs:domain rdf:resource="http://example.org/onto/class/google_dataplex_datascan"/>
    <rdfs:range rdf:resource="http://www.w3.org/2001/XMLSchema#string"/>
  </owl:DatatypeProperty>
  <owl:DatatypeProperty rdf:about="http://example.org/onto/prop/google_dataplex_datascan_results_table">
    <rdfs:label>results_table</rdfs:label>
    <rdfs:comment>The BigQuery table to export DataQualityScan results to.
Format://bigquery.googleapis.com/projects/PROJECT_ID/datasets/DATASET_ID/tables/TABLE_ID</rdfs:comment>
    <rdfs:domain rdf:resource="http://example.org/onto/class/google_dataplex_datascan"/>
    <rdfs:range rdf:resource="http://www.w3.org/2001/XMLSchema#string"/>
  </owl:DatatypeProperty>
  <owl:DatatypeProperty rdf:about="http://example.org/onto/prop/google_dataplex_datascan_emails">
    <rdfs:label>emails</rdfs:label>
    <rdfs:comment>The email recipients who will receive the DataQualityScan results report.</rdfs:comment>
    <rdfs:domain rdf:resource="http://example.org/onto/class/google_dataplex_datascan"/>
    <rdfs:range rdf:resource="http://www.w3.org/2001/XMLSchema#string"/>
  </owl:DatatypeProperty>
  <owl:DatatypeProperty rdf:about="http://example.org/onto/prop/google_dataplex_datascan_score_threshold">
    <rdfs:label>score_threshold</rdfs:label>
    <rdfs:comment>The score range is in [0,100].</rdfs:comment>
    <rdfs:domain rdf:resource="http://example.org/onto/class/google_dataplex_datascan"/>
    <rdfs:range rdf:resource="http://www.w3.org/2001/XMLSchema#string"/>
  </owl:DatatypeProperty>
  <owl:DatatypeProperty rdf:about="http://example.org/onto/prop/google_dataplex_datascan_column">
    <rdfs:label>column</rdfs:label>
    <rdfs:comment>The unnested column which this rule is evaluated against.</rdfs:comment>
    <rdfs:domain rdf:resource="http://example.org/onto/class/google_dataplex_datascan"/>
    <rdfs:range rdf:resource="http://www.w3.org/2001/XMLSchema#string"/>
  </owl:DatatypeProperty>
  <owl:DatatypeProperty rdf:about="http://example.org/onto/prop/google_dataplex_datascan_description">
    <rdfs:label>description</rdfs:label>
    <rdfs:comment>Description of the rule.
The maximum length is 1,024 characters.</rdfs:comment>
    <rdfs:domain rdf:resource="http://example.org/onto/class/google_dataplex_datascan"/>
    <rdfs:range rdf:resource="http://www.w3.org/2001/XMLSchema#string"/>
  </owl:DatatypeProperty>
  <owl:DatatypeProperty rdf:about="http://example.org/onto/prop/google_dataplex_datascan_dimension">
    <rdfs:label>dimension</rdfs:label>
    <rdfs:comment>The dimension name a rule belongs to. Custom dimension name is supported with all uppercase letters and maximum length of 30 characters.</rdfs:comment>
    <rdfs:domain rdf:resource="http://example.org/onto/class/google_dataplex_datascan"/>
    <rdfs:range rdf:resource="http://www.w3.org/2001/XMLSchema#string"/>
  </owl:DatatypeProperty>
  <owl:DatatypeProperty rdf:about="http://example.org/onto/prop/google_dataplex_datascan_ignore_null">
    <rdfs:label>ignore_null</rdfs:label>
    <rdfs:comment>Rows with null values will automatically fail a rule, unless ignoreNull is true. In that case, such null rows are trivially considered passing. Only applicable to ColumnMap rules.</rdfs:comment>
    <rdfs:domain rdf:resource="http://example.org/onto/class/google_dataplex_datascan"/>
    <rdfs:range rdf:resource="http://www.w3.org/2001/XMLSchema#string"/>
  </owl:DatatypeProperty>
  <owl:DatatypeProperty rdf:about="http://example.org/onto/prop/google_dataplex_datascan_name">
    <rdfs:label>name</rdfs:label>
    <rdfs:comment>A mutable name for the rule.
The name must contain only letters (a-z, A-Z), numbers (0-9), or hyphens (-).
The maximum length is 63 characters.
Must start with a letter.
Must end with a number or a letter.</rdfs:comment>
    <rdfs:domain rdf:resource="http://example.org/onto/class/google_dataplex_datascan"/>
    <rdfs:range rdf:resource="http://www.w3.org/2001/XMLSchema#string"/>
  </owl:DatatypeProperty>
  <owl:DatatypeProperty rdf:about="http://example.org/onto/prop/google_dataplex_datascan_suspended">
    <rdfs:label>suspended</rdfs:label>
    <rdfs:comment>Whether the Rule is active or suspended. Default = false.</rdfs:comment>
    <rdfs:domain rdf:resource="http://example.org/onto/class/google_dataplex_datascan"/>
    <rdfs:range rdf:resource="http://www.w3.org/2001/XMLSchema#string"/>
  </owl:DatatypeProperty>
  <owl:DatatypeProperty rdf:about="http://example.org/onto/prop/google_dataplex_datascan_threshold">
    <rdfs:label>threshold</rdfs:label>
    <rdfs:comment>The minimum ratio of passing_rows / total_rows required to pass this rule, with a range of [0.0, 1.0]. 0 indicates default value (i.e. 1.0).</rdfs:comment>
    <rdfs:domain rdf:resource="http://example.org/onto/class/google_dataplex_datascan"/>
    <rdfs:range rdf:resource="http://www.w3.org/2001/XMLSchema#string"/>
  </owl:DatatypeProperty>
  <owl:DatatypeProperty rdf:about="http://example.org/onto/prop/google_dataplex_datascan_max_value">
    <rdfs:label>max_value</rdfs:label>
    <rdfs:comment>The maximum column value allowed for a row to pass this validation. At least one of minValue and maxValue need to be provided.</rdfs:comment>
    <rdfs:domain rdf:resource="http://example.org/onto/class/google_dataplex_datascan"/>
    <rdfs:range rdf:resource="http://www.w3.org/2001/XMLSchema#string"/>
  </owl:DatatypeProperty>
  <owl:DatatypeProperty rdf:about="http://example.org/onto/prop/google_dataplex_datascan_min_value">
    <rdfs:label>min_value</rdfs:label>
    <rdfs:comment>The minimum column value allowed for a row to pass this validation. At least one of minValue and maxValue need to be provided.</rdfs:comment>
    <rdfs:domain rdf:resource="http://example.org/onto/class/google_dataplex_datascan"/>
    <rdfs:range rdf:resource="http://www.w3.org/2001/XMLSchema#string"/>
  </owl:DatatypeProperty>
  <owl:DatatypeProperty rdf:about="http://example.org/onto/prop/google_dataplex_datascan_strict_max_enabled">
    <rdfs:label>strict_max_enabled</rdfs:label>
    <rdfs:comment>Whether each value needs to be strictly lesser than ('<') the maximum, or if equality is allowed.
Only relevant if a maxValue has been defined. Default = false.</rdfs:comment>
    <rdfs:domain rdf:resource="http://example.org/onto/class/google_dataplex_datascan"/>
    <rdfs:range rdf:resource="http://www.w3.org/2001/XMLSchema#string"/>
  </owl:DatatypeProperty>
  <owl:DatatypeProperty rdf:about="http://example.org/onto/prop/google_dataplex_datascan_strict_min_enabled">
    <rdfs:label>strict_min_enabled</rdfs:label>
    <rdfs:comment>Whether each value needs to be strictly greater than ('>') the minimum, or if equality is allowed.
Only relevant if a minValue has been defined. Default = false.</rdfs:comment>
    <rdfs:domain rdf:resource="http://example.org/onto/class/google_dataplex_datascan"/>
    <rdfs:range rdf:resource="http://www.w3.org/2001/XMLSchema#string"/>
  </owl:DatatypeProperty>
  <owl:DatatypeProperty rdf:about="http://example.org/onto/prop/google_dataplex_datascan_regex">
    <rdfs:label>regex</rdfs:label>
    <rdfs:comment>A regular expression the column value is expected to match.</rdfs:comment>
    <rdfs:domain rdf:resource="http://example.org/onto/class/google_dataplex_datascan"/>
    <rdfs:range rdf:resource="http://www.w3.org/2001/XMLSchema#string"/>
  </owl:DatatypeProperty>
  <owl:DatatypeProperty rdf:about="http://example.org/onto/prop/google_dataplex_datascan_sql_expression">
    <rdfs:label>sql_expression</rdfs:label>
    <rdfs:comment>The SQL expression.</rdfs:comment>
    <rdfs:domain rdf:resource="http://example.org/onto/class/google_dataplex_datascan"/>
    <rdfs:range rdf:resource="http://www.w3.org/2001/XMLSchema#string"/>
  </owl:DatatypeProperty>
  <owl:DatatypeProperty rdf:about="http://example.org/onto/prop/google_dataplex_datascan_values">
    <rdfs:label>values</rdfs:label>
    <rdfs:comment>Expected values for the column value.</rdfs:comment>
    <rdfs:domain rdf:resource="http://example.org/onto/class/google_dataplex_datascan"/>
    <rdfs:range rdf:resource="http://www.w3.org/2001/XMLSchema#string"/>
  </owl:DatatypeProperty>
  <owl:DatatypeProperty rdf:about="http://example.org/onto/prop/google_dataplex_datascan_sql_statement">
    <rdfs:label>sql_statement</rdfs:label>
    <rdfs:comment>The SQL statement.</rdfs:comment>
    <rdfs:domain rdf:resource="http://example.org/onto/class/google_dataplex_datascan"/>
    <rdfs:range rdf:resource="http://www.w3.org/2001/XMLSchema#string"/>
  </owl:DatatypeProperty>
  <owl:DatatypeProperty rdf:about="http://example.org/onto/prop/google_dataplex_datascan_max_value">
    <rdfs:label>max_value</rdfs:label>
    <rdfs:comment>The maximum column statistic value allowed for a row to pass this validation.
At least one of minValue and maxValue need to be provided.</rdfs:comment>
    <rdfs:domain rdf:resource="http://example.org/onto/class/google_dataplex_datascan"/>
    <rdfs:range rdf:resource="http://www.w3.org/2001/XMLSchema#string"/>
  </owl:DatatypeProperty>
  <owl:DatatypeProperty rdf:about="http://example.org/onto/prop/google_dataplex_datascan_min_value">
    <rdfs:label>min_value</rdfs:label>
    <rdfs:comment>The minimum column statistic value allowed for a row to pass this validation.
At least one of minValue and maxValue need to be provided.</rdfs:comment>
    <rdfs:domain rdf:resource="http://example.org/onto/class/google_dataplex_datascan"/>
    <rdfs:range rdf:resource="http://www.w3.org/2001/XMLSchema#string"/>
  </owl:DatatypeProperty>
  <owl:DatatypeProperty rdf:about="http://example.org/onto/prop/google_dataplex_datascan_statistic">
    <rdfs:label>statistic</rdfs:label>
    <rdfs:comment>column statistics. Possible values: ["STATISTIC_UNDEFINED", "MEAN", "MIN", "MAX"]</rdfs:comment>
    <rdfs:domain rdf:resource="http://example.org/onto/class/google_dataplex_datascan"/>
    <rdfs:range rdf:resource="http://www.w3.org/2001/XMLSchema#string"/>
  </owl:DatatypeProperty>
  <owl:DatatypeProperty rdf:about="http://example.org/onto/prop/google_dataplex_datascan_strict_max_enabled">
    <rdfs:label>strict_max_enabled</rdfs:label>
    <rdfs:comment>Whether column statistic needs to be strictly lesser than ('<') the maximum, or if equality is allowed.
Only relevant if a maxValue has been defined. Default = false.</rdfs:comment>
    <rdfs:domain rdf:resource="http://example.org/onto/class/google_dataplex_datascan"/>
    <rdfs:range rdf:resource="http://www.w3.org/2001/XMLSchema#string"/>
  </owl:DatatypeProperty>
  <owl:DatatypeProperty rdf:about="http://example.org/onto/prop/google_dataplex_datascan_strict_min_enabled">
    <rdfs:label>strict_min_enabled</rdfs:label>
    <rdfs:comment>Whether column statistic needs to be strictly greater than ('>') the minimum, or if equality is allowed.
Only relevant if a minValue has been defined. Default = false.</rdfs:comment>
    <rdfs:domain rdf:resource="http://example.org/onto/class/google_dataplex_datascan"/>
    <rdfs:range rdf:resource="http://www.w3.org/2001/XMLSchema#string"/>
  </owl:DatatypeProperty>
  <owl:DatatypeProperty rdf:about="http://example.org/onto/prop/google_dataplex_datascan_sql_expression">
    <rdfs:label>sql_expression</rdfs:label>
    <rdfs:comment>The SQL expression.</rdfs:comment>
    <rdfs:domain rdf:resource="http://example.org/onto/class/google_dataplex_datascan"/>
    <rdfs:range rdf:resource="http://www.w3.org/2001/XMLSchema#string"/>
  </owl:DatatypeProperty>
  <owl:DatatypeProperty rdf:about="http://example.org/onto/prop/google_dataplex_datascan_field">
    <rdfs:label>field</rdfs:label>
    <rdfs:comment>The unnested field (of type Date or Timestamp) that contains values which monotonically increase over time. If not specified, a data scan will run for all data in the table.</rdfs:comment>
    <rdfs:domain rdf:resource="http://example.org/onto/class/google_dataplex_datascan"/>
    <rdfs:range rdf:resource="http://www.w3.org/2001/XMLSchema#string"/>
  </owl:DatatypeProperty>
  <owl:DatatypeProperty rdf:about="http://example.org/onto/prop/google_dataplex_datascan_cron">
    <rdfs:label>cron</rdfs:label>
    <rdfs:comment>Cron schedule for running scans periodically. This field is required for Schedule scans.</rdfs:comment>
    <rdfs:domain rdf:resource="http://example.org/onto/class/google_dataplex_datascan"/>
    <rdfs:range rdf:resource="http://www.w3.org/2001/XMLSchema#string"/>
  </owl:DatatypeProperty>
  <owl:DatatypeProperty rdf:about="http://example.org/onto/prop/google_dataplex_datascan_create">
    <rdfs:label>create</rdfs:label>
    <rdfs:domain rdf:resource="http://example.org/onto/class/google_dataplex_datascan"/>
    <rdfs:range rdf:resource="http://www.w3.org/2001/XMLSchema#string"/>
  </owl:DatatypeProperty>
  <owl:DatatypeProperty rdf:about="http://example.org/onto/prop/google_dataplex_datascan_delete">
    <rdfs:label>delete</rdfs:label>
    <rdfs:domain rdf:resource="http://example.org/onto/class/google_dataplex_datascan"/>
    <rdfs:range rdf:resource="http://www.w3.org/2001/XMLSchema#string"/>
  </owl:DatatypeProperty>
  <owl:DatatypeProperty rdf:about="http://example.org/onto/prop/google_dataplex_datascan_update">
    <rdfs:label>update</rdfs:label>
    <rdfs:domain rdf:resource="http://example.org/onto/class/google_dataplex_datascan"/>
    <rdfs:range rdf:resource="http://www.w3.org/2001/XMLSchema#string"/>
  </owl:DatatypeProperty>
</rdf:RDF>
