<?xml version="1.0" encoding="UTF-8"?>
<rdf:RDF
  xmlns:rdf="http://www.w3.org/1999/02/22-rdf-syntax-ns#"
  xmlns:rdfs="http://www.w3.org/2000/01/rdf-schema#"
  xmlns:owl="http://www.w3.org/2002/07/owl#"
  xmlns:xsd="http://www.w3.org/2001/XMLSchema#"
  xml:base="http://example.org/onto/">
  <owl:Class rdf:about="http://example.org/onto/class/google_kms_key_ring_import_job">
    <rdfs:label>google_kms_key_ring_import_job</rdfs:label>
    <rdfs:comment>#
#     ***     AUTO GENERATED CODE    ***    Type: MMv1     ***
#
# ----------------------------------------------------------------------------
#
#     This code is generated by Magic Modules using the following:
#
#     Configuration: https:#github.com/GoogleCloudPlatform/magic-modules/tree/main/mmv1/products/kms/KeyRingImportJob.yaml
#     Template:      https:#github.com/GoogleCloudPlatform/magic-modules/tree/main/mmv1/templates/terraform/resource.html.markdown.tmpl
#
#     DO NOT EDIT this file directly. Any changes made to this file will be
#     overwritten during the next generation cycle.
#
# ----------------------------------------------------------------------------
subcategory: "Cloud Key Management Service"
description: |-
  A `KeyRingImportJob` can be used to create `CryptoKeys` and `CryptoKeyVersions` using pre-existing
  key material, generated outside of Cloud KMS.
---</rdfs:comment>
  </owl:Class>
  <owl:DatatypeProperty rdf:about="http://example.org/onto/prop/google_kms_key_ring_import_job_attestation">
    <rdfs:label>attestation</rdfs:label>
    <rdfs:comment>Statement that was generated and signed by the key creator (for example, an HSM) at key creation time.
Use this statement to verify attributes of the key as stored on the HSM, independently of Google.
Only present if the chosen ImportMethod is one with a protection level of HSM.</rdfs:comment>
    <rdfs:domain rdf:resource="http://example.org/onto/class/google_kms_key_ring_import_job"/>
    <rdfs:range rdf:resource="http://www.w3.org/2001/XMLSchema#string"/>
  </owl:DatatypeProperty>
  <owl:DatatypeProperty rdf:about="http://example.org/onto/prop/google_kms_key_ring_import_job_expire_time">
    <rdfs:label>expire_time</rdfs:label>
    <rdfs:comment>The time at which this resource is scheduled for expiration and can no longer be used.
This is in RFC3339 text format.</rdfs:comment>
    <rdfs:domain rdf:resource="http://example.org/onto/class/google_kms_key_ring_import_job"/>
    <rdfs:range rdf:resource="http://www.w3.org/2001/XMLSchema#string"/>
  </owl:DatatypeProperty>
  <owl:DatatypeProperty rdf:about="http://example.org/onto/prop/google_kms_key_ring_import_job_id">
    <rdfs:label>id</rdfs:label>
    <rdfs:domain rdf:resource="http://example.org/onto/class/google_kms_key_ring_import_job"/>
    <rdfs:range rdf:resource="http://www.w3.org/2001/XMLSchema#string"/>
  </owl:DatatypeProperty>
  <owl:DatatypeProperty rdf:about="http://example.org/onto/prop/google_kms_key_ring_import_job_import_job_id">
    <rdfs:label>import_job_id</rdfs:label>
    <rdfs:comment>It must be unique within a KeyRing and match the regular expression [a-zA-Z0-9_-]{1,63}</rdfs:comment>
    <rdfs:domain rdf:resource="http://example.org/onto/class/google_kms_key_ring_import_job"/>
    <rdfs:range rdf:resource="http://www.w3.org/2001/XMLSchema#string"/>
  </owl:DatatypeProperty>
  <owl:DatatypeProperty rdf:about="http://example.org/onto/prop/google_kms_key_ring_import_job_import_method">
    <rdfs:label>import_method</rdfs:label>
    <rdfs:comment>The wrapping method to be used for incoming key material. Possible values: ["RSA_OAEP_3072_SHA1_AES_256", "RSA_OAEP_4096_SHA1_AES_256", "RSA_OAEP_3072_SHA256_AES_256", "RSA_OAEP_4096_SHA256_AES_256", "RSA_OAEP_3072_SHA256", "RSA_OAEP_4096_SHA256"]</rdfs:comment>
    <rdfs:domain rdf:resource="http://example.org/onto/class/google_kms_key_ring_import_job"/>
    <rdfs:range rdf:resource="http://www.w3.org/2001/XMLSchema#string"/>
  </owl:DatatypeProperty>
  <owl:DatatypeProperty rdf:about="http://example.org/onto/prop/google_kms_key_ring_import_job_key_ring">
    <rdfs:label>key_ring</rdfs:label>
    <rdfs:comment>The KeyRing that this import job belongs to.
Format: ''projects/{{project}}/locations/{{location}}/keyRings/{{keyRing}}''.</rdfs:comment>
    <rdfs:domain rdf:resource="http://example.org/onto/class/google_kms_key_ring_import_job"/>
    <rdfs:range rdf:resource="http://www.w3.org/2001/XMLSchema#string"/>
  </owl:DatatypeProperty>
  <owl:DatatypeProperty rdf:about="http://example.org/onto/prop/google_kms_key_ring_import_job_name">
    <rdfs:label>name</rdfs:label>
    <rdfs:comment>The resource name for this ImportJob in the format projects/*/locations/*/keyRings/*/importJobs/*.</rdfs:comment>
    <rdfs:domain rdf:resource="http://example.org/onto/class/google_kms_key_ring_import_job"/>
    <rdfs:range rdf:resource="http://www.w3.org/2001/XMLSchema#string"/>
  </owl:DatatypeProperty>
  <owl:DatatypeProperty rdf:about="http://example.org/onto/prop/google_kms_key_ring_import_job_protection_level">
    <rdfs:label>protection_level</rdfs:label>
    <rdfs:comment>The protection level of the ImportJob. This must match the protectionLevel of the
versionTemplate on the CryptoKey you attempt to import into. Possible values: ["SOFTWARE", "HSM", "EXTERNAL"]</rdfs:comment>
    <rdfs:domain rdf:resource="http://example.org/onto/class/google_kms_key_ring_import_job"/>
    <rdfs:range rdf:resource="http://www.w3.org/2001/XMLSchema#string"/>
  </owl:DatatypeProperty>
  <owl:DatatypeProperty rdf:about="http://example.org/onto/prop/google_kms_key_ring_import_job_public_key">
    <rdfs:label>public_key</rdfs:label>
    <rdfs:comment>The public key with which to wrap key material prior to import. Only returned if state is 'ACTIVE'.</rdfs:comment>
    <rdfs:domain rdf:resource="http://example.org/onto/class/google_kms_key_ring_import_job"/>
    <rdfs:range rdf:resource="http://www.w3.org/2001/XMLSchema#string"/>
  </owl:DatatypeProperty>
  <owl:DatatypeProperty rdf:about="http://example.org/onto/prop/google_kms_key_ring_import_job_state">
    <rdfs:label>state</rdfs:label>
    <rdfs:comment>The current state of the ImportJob, indicating if it can be used.</rdfs:comment>
    <rdfs:domain rdf:resource="http://example.org/onto/class/google_kms_key_ring_import_job"/>
    <rdfs:range rdf:resource="http://www.w3.org/2001/XMLSchema#string"/>
  </owl:DatatypeProperty>
  <owl:DatatypeProperty rdf:about="http://example.org/onto/prop/google_kms_key_ring_import_job_create">
    <rdfs:label>create</rdfs:label>
    <rdfs:domain rdf:resource="http://example.org/onto/class/google_kms_key_ring_import_job"/>
    <rdfs:range rdf:resource="http://www.w3.org/2001/XMLSchema#string"/>
  </owl:DatatypeProperty>
  <owl:DatatypeProperty rdf:about="http://example.org/onto/prop/google_kms_key_ring_import_job_delete">
    <rdfs:label>delete</rdfs:label>
    <rdfs:domain rdf:resource="http://example.org/onto/class/google_kms_key_ring_import_job"/>
    <rdfs:range rdf:resource="http://www.w3.org/2001/XMLSchema#string"/>
  </owl:DatatypeProperty>
</rdf:RDF>
