<?xml version="1.0" encoding="UTF-8"?>
<rdf:RDF
  xmlns:rdf="http://www.w3.org/1999/02/22-rdf-syntax-ns#"
  xmlns:rdfs="http://www.w3.org/2000/01/rdf-schema#"
  xmlns:owl="http://www.w3.org/2002/07/owl#"
  xmlns:xsd="http://www.w3.org/2001/XMLSchema#"
  xml:base="http://example.org/onto/">
  <owl:Class rdf:about="http://example.org/onto/class/google_resource_manager_lien">
    <rdfs:label>google_resource_manager_lien</rdfs:label>
    <rdfs:comment>#
#     ***     AUTO GENERATED CODE    ***    Type: MMv1     ***
#
# ----------------------------------------------------------------------------
#
#     This code is generated by Magic Modules using the following:
#
#     Configuration: https:#github.com/GoogleCloudPlatform/magic-modules/tree/main/mmv1/products/resourcemanager/Lien.yaml
#     Template:      https:#github.com/GoogleCloudPlatform/magic-modules/tree/main/mmv1/templates/terraform/resource.html.markdown.tmpl
#
#     DO NOT EDIT this file directly. Any changes made to this file will be
#     overwritten during the next generation cycle.
#
# ----------------------------------------------------------------------------
subcategory: "Resource Manager"
description: |-
  A Lien represents an encumbrance on the actions that can be performed on a resource.
---</rdfs:comment>
  </owl:Class>
  <owl:DatatypeProperty rdf:about="http://example.org/onto/prop/google_resource_manager_lien_create_time">
    <rdfs:label>create_time</rdfs:label>
    <rdfs:comment>Time of creation</rdfs:comment>
    <rdfs:domain rdf:resource="http://example.org/onto/class/google_resource_manager_lien"/>
    <rdfs:range rdf:resource="http://www.w3.org/2001/XMLSchema#string"/>
  </owl:DatatypeProperty>
  <owl:DatatypeProperty rdf:about="http://example.org/onto/prop/google_resource_manager_lien_id">
    <rdfs:label>id</rdfs:label>
    <rdfs:domain rdf:resource="http://example.org/onto/class/google_resource_manager_lien"/>
    <rdfs:range rdf:resource="http://www.w3.org/2001/XMLSchema#string"/>
  </owl:DatatypeProperty>
  <owl:DatatypeProperty rdf:about="http://example.org/onto/prop/google_resource_manager_lien_name">
    <rdfs:label>name</rdfs:label>
    <rdfs:comment>A system-generated unique identifier for this Lien.</rdfs:comment>
    <rdfs:domain rdf:resource="http://example.org/onto/class/google_resource_manager_lien"/>
    <rdfs:range rdf:resource="http://www.w3.org/2001/XMLSchema#string"/>
  </owl:DatatypeProperty>
  <owl:DatatypeProperty rdf:about="http://example.org/onto/prop/google_resource_manager_lien_origin">
    <rdfs:label>origin</rdfs:label>
    <rdfs:comment>A stable, user-visible/meaningful string identifying the origin
of the Lien, intended to be inspected programmatically. Maximum length of
200 characters.</rdfs:comment>
    <rdfs:domain rdf:resource="http://example.org/onto/class/google_resource_manager_lien"/>
    <rdfs:range rdf:resource="http://www.w3.org/2001/XMLSchema#string"/>
  </owl:DatatypeProperty>
  <owl:DatatypeProperty rdf:about="http://example.org/onto/prop/google_resource_manager_lien_parent">
    <rdfs:label>parent</rdfs:label>
    <rdfs:comment>A reference to the resource this Lien is attached to.
The server will validate the parent against those for which Liens are supported.
Since a variety of objects can have Liens against them, you must provide the type
prefix (e.g. "projects/my-project-name").</rdfs:comment>
    <rdfs:domain rdf:resource="http://example.org/onto/class/google_resource_manager_lien"/>
    <rdfs:range rdf:resource="http://www.w3.org/2001/XMLSchema#string"/>
  </owl:DatatypeProperty>
  <owl:DatatypeProperty rdf:about="http://example.org/onto/prop/google_resource_manager_lien_reason">
    <rdfs:label>reason</rdfs:label>
    <rdfs:comment>Concise user-visible strings indicating why an action cannot be performed
on a resource. Maximum length of 200 characters.</rdfs:comment>
    <rdfs:domain rdf:resource="http://example.org/onto/class/google_resource_manager_lien"/>
    <rdfs:range rdf:resource="http://www.w3.org/2001/XMLSchema#string"/>
  </owl:DatatypeProperty>
  <owl:DatatypeProperty rdf:about="http://example.org/onto/prop/google_resource_manager_lien_restrictions">
    <rdfs:label>restrictions</rdfs:label>
    <rdfs:comment>The types of operations which should be blocked as a result of this Lien.
Each value should correspond to an IAM permission. The server will validate
the permissions against those for which Liens are supported.  An empty
list is meaningless and will be rejected.
e.g. ['resourcemanager.projects.delete']</rdfs:comment>
    <rdfs:domain rdf:resource="http://example.org/onto/class/google_resource_manager_lien"/>
    <rdfs:range rdf:resource="http://www.w3.org/2001/XMLSchema#string"/>
  </owl:DatatypeProperty>
  <owl:DatatypeProperty rdf:about="http://example.org/onto/prop/google_resource_manager_lien_create">
    <rdfs:label>create</rdfs:label>
    <rdfs:domain rdf:resource="http://example.org/onto/class/google_resource_manager_lien"/>
    <rdfs:range rdf:resource="http://www.w3.org/2001/XMLSchema#string"/>
  </owl:DatatypeProperty>
  <owl:DatatypeProperty rdf:about="http://example.org/onto/prop/google_resource_manager_lien_delete">
    <rdfs:label>delete</rdfs:label>
    <rdfs:domain rdf:resource="http://example.org/onto/class/google_resource_manager_lien"/>
    <rdfs:range rdf:resource="http://www.w3.org/2001/XMLSchema#string"/>
  </owl:DatatypeProperty>
</rdf:RDF>
