<?xml version="1.0" encoding="UTF-8"?>
<rdf:RDF
  xmlns:rdf="http://www.w3.org/1999/02/22-rdf-syntax-ns#"
  xmlns:rdfs="http://www.w3.org/2000/01/rdf-schema#"
  xmlns:owl="http://www.w3.org/2002/07/owl#"
  xmlns:xsd="http://www.w3.org/2001/XMLSchema#"
  xml:base="http://example.org/onto/">
  <owl:Class rdf:about="http://example.org/onto/class/google_alloydb_cluster">
    <rdfs:label>google_alloydb_cluster</rdfs:label>
    <rdfs:comment>#
#     ***     AUTO GENERATED CODE    ***    Type: MMv1     ***
#
# ----------------------------------------------------------------------------
#
#     This code is generated by Magic Modules using the following:
#
#     Configuration: https:#github.com/GoogleCloudPlatform/magic-modules/tree/main/mmv1/products/alloydb/Cluster.yaml
#     Template:      https:#github.com/GoogleCloudPlatform/magic-modules/tree/main/mmv1/templates/terraform/resource.html.markdown.tmpl
#
#     DO NOT EDIT this file directly. Any changes made to this file will be
#     overwritten during the next generation cycle.
#
# ----------------------------------------------------------------------------
subcategory: "AlloyDB"
description: |-
  A managed alloydb cluster.
---</rdfs:comment>
  </owl:Class>
  <owl:DatatypeProperty rdf:about="http://example.org/onto/prop/google_alloydb_cluster_annotations">
    <rdfs:label>annotations</rdfs:label>
    <rdfs:comment>Annotations to allow client tools to store small amount of arbitrary data. This is distinct from labels. https://google.aip.dev/128
An object containing a list of "key": value pairs. Example: { "name": "wrench", "mass": "1.3kg", "count": "3" }.


**Note**: This field is non-authoritative, and will only manage the annotations present in your configuration.
Please refer to the field 'effective_annotations' for all of the annotations present on the resource.</rdfs:comment>
    <rdfs:domain rdf:resource="http://example.org/onto/class/google_alloydb_cluster"/>
    <rdfs:range rdf:resource="http://www.w3.org/2001/XMLSchema#string"/>
  </owl:DatatypeProperty>
  <owl:DatatypeProperty rdf:about="http://example.org/onto/prop/google_alloydb_cluster_backup_source">
    <rdfs:label>backup_source</rdfs:label>
    <rdfs:comment>Cluster created from backup.</rdfs:comment>
    <rdfs:domain rdf:resource="http://example.org/onto/class/google_alloydb_cluster"/>
    <rdfs:range rdf:resource="http://www.w3.org/2001/XMLSchema#string"/>
  </owl:DatatypeProperty>
  <owl:DatatypeProperty rdf:about="http://example.org/onto/prop/google_alloydb_cluster_cluster_id">
    <rdfs:label>cluster_id</rdfs:label>
    <rdfs:comment>The ID of the alloydb cluster.</rdfs:comment>
    <rdfs:domain rdf:resource="http://example.org/onto/class/google_alloydb_cluster"/>
    <rdfs:range rdf:resource="http://www.w3.org/2001/XMLSchema#string"/>
  </owl:DatatypeProperty>
  <owl:DatatypeProperty rdf:about="http://example.org/onto/prop/google_alloydb_cluster_cluster_type">
    <rdfs:label>cluster_type</rdfs:label>
    <rdfs:comment>The type of cluster. If not set, defaults to PRIMARY. Default value: "PRIMARY" Possible values: ["PRIMARY", "SECONDARY"]</rdfs:comment>
    <rdfs:domain rdf:resource="http://example.org/onto/class/google_alloydb_cluster"/>
    <rdfs:range rdf:resource="http://www.w3.org/2001/XMLSchema#string"/>
  </owl:DatatypeProperty>
  <owl:DatatypeProperty rdf:about="http://example.org/onto/prop/google_alloydb_cluster_continuous_backup_info">
    <rdfs:label>continuous_backup_info</rdfs:label>
    <rdfs:comment>ContinuousBackupInfo describes the continuous backup properties of a cluster.</rdfs:comment>
    <rdfs:domain rdf:resource="http://example.org/onto/class/google_alloydb_cluster"/>
    <rdfs:range rdf:resource="http://www.w3.org/2001/XMLSchema#string"/>
  </owl:DatatypeProperty>
  <owl:DatatypeProperty rdf:about="http://example.org/onto/prop/google_alloydb_cluster_database_version">
    <rdfs:label>database_version</rdfs:label>
    <rdfs:comment>The database engine major version. This is an optional field and it's populated at the Cluster creation time.
Note: Changing this field to a higer version results in upgrading the AlloyDB cluster which is an irreversible change.</rdfs:comment>
    <rdfs:domain rdf:resource="http://example.org/onto/class/google_alloydb_cluster"/>
    <rdfs:range rdf:resource="http://www.w3.org/2001/XMLSchema#string"/>
  </owl:DatatypeProperty>
  <owl:DatatypeProperty rdf:about="http://example.org/onto/prop/google_alloydb_cluster_deletion_policy">
    <rdfs:label>deletion_policy</rdfs:label>
    <rdfs:comment>Policy to determine if the cluster should be deleted forcefully.
Deleting a cluster forcefully, deletes the cluster and all its associated instances within the cluster.
Deleting a Secondary cluster with a secondary instance REQUIRES setting deletion_policy = "FORCE" otherwise an error is returned. This is needed as there is no support to delete just the secondary instance, and the only way to delete secondary instance is to delete the associated secondary cluster forcefully which also deletes the secondary instance.
Possible values: DEFAULT, FORCE</rdfs:comment>
    <rdfs:domain rdf:resource="http://example.org/onto/class/google_alloydb_cluster"/>
    <rdfs:range rdf:resource="http://www.w3.org/2001/XMLSchema#string"/>
  </owl:DatatypeProperty>
  <owl:DatatypeProperty rdf:about="http://example.org/onto/prop/google_alloydb_cluster_deletion_protection">
    <rdfs:label>deletion_protection</rdfs:label>
    <rdfs:comment>Whether Terraform will be prevented from destroying the cluster.
When the field is set to true or unset in Terraform state, a 'terraform apply'
or 'terraform destroy' that would delete the cluster will fail.
When the field is set to false, deleting the cluster is allowed.</rdfs:comment>
    <rdfs:domain rdf:resource="http://example.org/onto/class/google_alloydb_cluster"/>
    <rdfs:range rdf:resource="http://www.w3.org/2001/XMLSchema#string"/>
  </owl:DatatypeProperty>
  <owl:DatatypeProperty rdf:about="http://example.org/onto/prop/google_alloydb_cluster_display_name">
    <rdfs:label>display_name</rdfs:label>
    <rdfs:comment>User-settable and human-readable display name for the Cluster.</rdfs:comment>
    <rdfs:domain rdf:resource="http://example.org/onto/class/google_alloydb_cluster"/>
    <rdfs:range rdf:resource="http://www.w3.org/2001/XMLSchema#string"/>
  </owl:DatatypeProperty>
  <owl:DatatypeProperty rdf:about="http://example.org/onto/prop/google_alloydb_cluster_effective_annotations">
    <rdfs:label>effective_annotations</rdfs:label>
    <rdfs:comment>All of annotations (key/value pairs) present on the resource in GCP, including the annotations configured through Terraform, other clients and services.</rdfs:comment>
    <rdfs:domain rdf:resource="http://example.org/onto/class/google_alloydb_cluster"/>
    <rdfs:range rdf:resource="http://www.w3.org/2001/XMLSchema#string"/>
  </owl:DatatypeProperty>
  <owl:DatatypeProperty rdf:about="http://example.org/onto/prop/google_alloydb_cluster_effective_labels">
    <rdfs:label>effective_labels</rdfs:label>
    <rdfs:comment>All of labels (key/value pairs) present on the resource in GCP, including the labels configured through Terraform, other clients and services.</rdfs:comment>
    <rdfs:domain rdf:resource="http://example.org/onto/class/google_alloydb_cluster"/>
    <rdfs:range rdf:resource="http://www.w3.org/2001/XMLSchema#string"/>
  </owl:DatatypeProperty>
  <owl:DatatypeProperty rdf:about="http://example.org/onto/prop/google_alloydb_cluster_encryption_info">
    <rdfs:label>encryption_info</rdfs:label>
    <rdfs:comment>EncryptionInfo describes the encryption information of a cluster or a backup.</rdfs:comment>
    <rdfs:domain rdf:resource="http://example.org/onto/class/google_alloydb_cluster"/>
    <rdfs:range rdf:resource="http://www.w3.org/2001/XMLSchema#string"/>
  </owl:DatatypeProperty>
  <owl:DatatypeProperty rdf:about="http://example.org/onto/prop/google_alloydb_cluster_etag">
    <rdfs:label>etag</rdfs:label>
    <rdfs:comment>For Resource freshness validation (https://google.aip.dev/154)</rdfs:comment>
    <rdfs:domain rdf:resource="http://example.org/onto/class/google_alloydb_cluster"/>
    <rdfs:range rdf:resource="http://www.w3.org/2001/XMLSchema#string"/>
  </owl:DatatypeProperty>
  <owl:DatatypeProperty rdf:about="http://example.org/onto/prop/google_alloydb_cluster_id">
    <rdfs:label>id</rdfs:label>
    <rdfs:domain rdf:resource="http://example.org/onto/class/google_alloydb_cluster"/>
    <rdfs:range rdf:resource="http://www.w3.org/2001/XMLSchema#string"/>
  </owl:DatatypeProperty>
  <owl:DatatypeProperty rdf:about="http://example.org/onto/prop/google_alloydb_cluster_labels">
    <rdfs:label>labels</rdfs:label>
    <rdfs:comment>User-defined labels for the alloydb cluster.

**Note**: This field is non-authoritative, and will only manage the labels present in your configuration.
Please refer to the field 'effective_labels' for all of the labels present on the resource.</rdfs:comment>
    <rdfs:domain rdf:resource="http://example.org/onto/class/google_alloydb_cluster"/>
    <rdfs:range rdf:resource="http://www.w3.org/2001/XMLSchema#string"/>
  </owl:DatatypeProperty>
  <owl:DatatypeProperty rdf:about="http://example.org/onto/prop/google_alloydb_cluster_location">
    <rdfs:label>location</rdfs:label>
    <rdfs:comment>The location where the alloydb cluster should reside.</rdfs:comment>
    <rdfs:domain rdf:resource="http://example.org/onto/class/google_alloydb_cluster"/>
    <rdfs:range rdf:resource="http://www.w3.org/2001/XMLSchema#string"/>
  </owl:DatatypeProperty>
  <owl:DatatypeProperty rdf:about="http://example.org/onto/prop/google_alloydb_cluster_migration_source">
    <rdfs:label>migration_source</rdfs:label>
    <rdfs:comment>Cluster created via DMS migration.</rdfs:comment>
    <rdfs:domain rdf:resource="http://example.org/onto/class/google_alloydb_cluster"/>
    <rdfs:range rdf:resource="http://www.w3.org/2001/XMLSchema#string"/>
  </owl:DatatypeProperty>
  <owl:DatatypeProperty rdf:about="http://example.org/onto/prop/google_alloydb_cluster_name">
    <rdfs:label>name</rdfs:label>
    <rdfs:comment>The name of the cluster resource.</rdfs:comment>
    <rdfs:domain rdf:resource="http://example.org/onto/class/google_alloydb_cluster"/>
    <rdfs:range rdf:resource="http://www.w3.org/2001/XMLSchema#string"/>
  </owl:DatatypeProperty>
  <owl:DatatypeProperty rdf:about="http://example.org/onto/prop/google_alloydb_cluster_project">
    <rdfs:label>project</rdfs:label>
    <rdfs:domain rdf:resource="http://example.org/onto/class/google_alloydb_cluster"/>
    <rdfs:range rdf:resource="http://www.w3.org/2001/XMLSchema#string"/>
  </owl:DatatypeProperty>
  <owl:DatatypeProperty rdf:about="http://example.org/onto/prop/google_alloydb_cluster_reconciling">
    <rdfs:label>reconciling</rdfs:label>
    <rdfs:comment>Output only. Reconciling (https://google.aip.dev/128#reconciliation).
Set to true if the current state of Cluster does not match the user's intended state, and the service is actively updating the resource to reconcile them.
This can happen due to user-triggered updates or system actions like failover or maintenance.</rdfs:comment>
    <rdfs:domain rdf:resource="http://example.org/onto/class/google_alloydb_cluster"/>
    <rdfs:range rdf:resource="http://www.w3.org/2001/XMLSchema#string"/>
  </owl:DatatypeProperty>
  <owl:DatatypeProperty rdf:about="http://example.org/onto/prop/google_alloydb_cluster_skip_await_major_version_upgrade">
    <rdfs:label>skip_await_major_version_upgrade</rdfs:label>
    <rdfs:comment>Set to true to skip awaiting on the major version upgrade of the cluster.
Possible values: true, false
Default value: "true"</rdfs:comment>
    <rdfs:domain rdf:resource="http://example.org/onto/class/google_alloydb_cluster"/>
    <rdfs:range rdf:resource="http://www.w3.org/2001/XMLSchema#string"/>
  </owl:DatatypeProperty>
  <owl:DatatypeProperty rdf:about="http://example.org/onto/prop/google_alloydb_cluster_state">
    <rdfs:label>state</rdfs:label>
    <rdfs:comment>Output only. The current serving state of the cluster.</rdfs:comment>
    <rdfs:domain rdf:resource="http://example.org/onto/class/google_alloydb_cluster"/>
    <rdfs:range rdf:resource="http://www.w3.org/2001/XMLSchema#string"/>
  </owl:DatatypeProperty>
  <owl:DatatypeProperty rdf:about="http://example.org/onto/prop/google_alloydb_cluster_subscription_type">
    <rdfs:label>subscription_type</rdfs:label>
    <rdfs:comment>The subscrition type of cluster. Possible values: ["TRIAL", "STANDARD"]</rdfs:comment>
    <rdfs:domain rdf:resource="http://example.org/onto/class/google_alloydb_cluster"/>
    <rdfs:range rdf:resource="http://www.w3.org/2001/XMLSchema#string"/>
  </owl:DatatypeProperty>
  <owl:DatatypeProperty rdf:about="http://example.org/onto/prop/google_alloydb_cluster_terraform_labels">
    <rdfs:label>terraform_labels</rdfs:label>
    <rdfs:comment>The combination of labels configured directly on the resource
 and default labels configured on the provider.</rdfs:comment>
    <rdfs:domain rdf:resource="http://example.org/onto/class/google_alloydb_cluster"/>
    <rdfs:range rdf:resource="http://www.w3.org/2001/XMLSchema#string"/>
  </owl:DatatypeProperty>
  <owl:DatatypeProperty rdf:about="http://example.org/onto/prop/google_alloydb_cluster_trial_metadata">
    <rdfs:label>trial_metadata</rdfs:label>
    <rdfs:comment>Contains information and all metadata related to TRIAL clusters.</rdfs:comment>
    <rdfs:domain rdf:resource="http://example.org/onto/class/google_alloydb_cluster"/>
    <rdfs:range rdf:resource="http://www.w3.org/2001/XMLSchema#string"/>
  </owl:DatatypeProperty>
  <owl:DatatypeProperty rdf:about="http://example.org/onto/prop/google_alloydb_cluster_uid">
    <rdfs:label>uid</rdfs:label>
    <rdfs:comment>The system-generated UID of the resource.</rdfs:comment>
    <rdfs:domain rdf:resource="http://example.org/onto/class/google_alloydb_cluster"/>
    <rdfs:range rdf:resource="http://www.w3.org/2001/XMLSchema#string"/>
  </owl:DatatypeProperty>
  <owl:DatatypeProperty rdf:about="http://example.org/onto/prop/google_alloydb_cluster_backup_window">
    <rdfs:label>backup_window</rdfs:label>
    <rdfs:comment>The length of the time window during which a backup can be taken. If a backup does not succeed within this time window, it will be canceled and considered failed.

The backup window must be at least 5 minutes long. There is no upper bound on the window. If not set, it will default to 1 hour.

A duration in seconds with up to nine fractional digits, terminated by 's'. Example: "3.5s".</rdfs:comment>
    <rdfs:domain rdf:resource="http://example.org/onto/class/google_alloydb_cluster"/>
    <rdfs:range rdf:resource="http://www.w3.org/2001/XMLSchema#string"/>
  </owl:DatatypeProperty>
  <owl:DatatypeProperty rdf:about="http://example.org/onto/prop/google_alloydb_cluster_enabled">
    <rdfs:label>enabled</rdfs:label>
    <rdfs:comment>Whether automated backups are enabled.</rdfs:comment>
    <rdfs:domain rdf:resource="http://example.org/onto/class/google_alloydb_cluster"/>
    <rdfs:range rdf:resource="http://www.w3.org/2001/XMLSchema#string"/>
  </owl:DatatypeProperty>
  <owl:DatatypeProperty rdf:about="http://example.org/onto/prop/google_alloydb_cluster_labels">
    <rdfs:label>labels</rdfs:label>
    <rdfs:comment>Labels to apply to backups created using this configuration.</rdfs:comment>
    <rdfs:domain rdf:resource="http://example.org/onto/class/google_alloydb_cluster"/>
    <rdfs:range rdf:resource="http://www.w3.org/2001/XMLSchema#string"/>
  </owl:DatatypeProperty>
  <owl:DatatypeProperty rdf:about="http://example.org/onto/prop/google_alloydb_cluster_location">
    <rdfs:label>location</rdfs:label>
    <rdfs:comment>The location where the backup will be stored. Currently, the only supported option is to store the backup in the same region as the cluster.</rdfs:comment>
    <rdfs:domain rdf:resource="http://example.org/onto/class/google_alloydb_cluster"/>
    <rdfs:range rdf:resource="http://www.w3.org/2001/XMLSchema#string"/>
  </owl:DatatypeProperty>
  <owl:DatatypeProperty rdf:about="http://example.org/onto/prop/google_alloydb_cluster_kms_key_name">
    <rdfs:label>kms_key_name</rdfs:label>
    <rdfs:comment>The fully-qualified resource name of the KMS key. Each Cloud KMS key is regionalized and has the following format: projects/[PROJECT]/locations/[REGION]/keyRings/[RING]/cryptoKeys/[KEY_NAME].</rdfs:comment>
    <rdfs:domain rdf:resource="http://example.org/onto/class/google_alloydb_cluster"/>
    <rdfs:range rdf:resource="http://www.w3.org/2001/XMLSchema#string"/>
  </owl:DatatypeProperty>
  <owl:DatatypeProperty rdf:about="http://example.org/onto/prop/google_alloydb_cluster_count">
    <rdfs:label>count</rdfs:label>
    <rdfs:comment>The number of backups to retain.</rdfs:comment>
    <rdfs:domain rdf:resource="http://example.org/onto/class/google_alloydb_cluster"/>
    <rdfs:range rdf:resource="http://www.w3.org/2001/XMLSchema#string"/>
  </owl:DatatypeProperty>
  <owl:DatatypeProperty rdf:about="http://example.org/onto/prop/google_alloydb_cluster_retention_period">
    <rdfs:label>retention_period</rdfs:label>
    <rdfs:comment>The retention period.
A duration in seconds with up to nine fractional digits, terminated by 's'. Example: "3.5s".</rdfs:comment>
    <rdfs:domain rdf:resource="http://example.org/onto/class/google_alloydb_cluster"/>
    <rdfs:range rdf:resource="http://www.w3.org/2001/XMLSchema#string"/>
  </owl:DatatypeProperty>
  <owl:DatatypeProperty rdf:about="http://example.org/onto/prop/google_alloydb_cluster_days_of_week">
    <rdfs:label>days_of_week</rdfs:label>
    <rdfs:comment>The days of the week to perform a backup. At least one day of the week must be provided. Possible values: ["MONDAY", "TUESDAY", "WEDNESDAY", "THURSDAY", "FRIDAY", "SATURDAY", "SUNDAY"]</rdfs:comment>
    <rdfs:domain rdf:resource="http://example.org/onto/class/google_alloydb_cluster"/>
    <rdfs:range rdf:resource="http://www.w3.org/2001/XMLSchema#string"/>
  </owl:DatatypeProperty>
  <owl:DatatypeProperty rdf:about="http://example.org/onto/prop/google_alloydb_cluster_hours">
    <rdfs:label>hours</rdfs:label>
    <rdfs:comment>Hours of day in 24 hour format. Should be from 0 to 23. An API may choose to allow the value "24:00:00" for scenarios like business closing time.</rdfs:comment>
    <rdfs:domain rdf:resource="http://example.org/onto/class/google_alloydb_cluster"/>
    <rdfs:range rdf:resource="http://www.w3.org/2001/XMLSchema#string"/>
  </owl:DatatypeProperty>
  <owl:DatatypeProperty rdf:about="http://example.org/onto/prop/google_alloydb_cluster_minutes">
    <rdfs:label>minutes</rdfs:label>
    <rdfs:comment>Minutes of hour of day. Currently, only the value 0 is supported.</rdfs:comment>
    <rdfs:domain rdf:resource="http://example.org/onto/class/google_alloydb_cluster"/>
    <rdfs:range rdf:resource="http://www.w3.org/2001/XMLSchema#string"/>
  </owl:DatatypeProperty>
  <owl:DatatypeProperty rdf:about="http://example.org/onto/prop/google_alloydb_cluster_nanos">
    <rdfs:label>nanos</rdfs:label>
    <rdfs:comment>Fractions of seconds in nanoseconds. Currently, only the value 0 is supported.</rdfs:comment>
    <rdfs:domain rdf:resource="http://example.org/onto/class/google_alloydb_cluster"/>
    <rdfs:range rdf:resource="http://www.w3.org/2001/XMLSchema#string"/>
  </owl:DatatypeProperty>
  <owl:DatatypeProperty rdf:about="http://example.org/onto/prop/google_alloydb_cluster_seconds">
    <rdfs:label>seconds</rdfs:label>
    <rdfs:comment>Seconds of minutes of the time. Currently, only the value 0 is supported.</rdfs:comment>
    <rdfs:domain rdf:resource="http://example.org/onto/class/google_alloydb_cluster"/>
    <rdfs:range rdf:resource="http://www.w3.org/2001/XMLSchema#string"/>
  </owl:DatatypeProperty>
  <owl:DatatypeProperty rdf:about="http://example.org/onto/prop/google_alloydb_cluster_enabled">
    <rdfs:label>enabled</rdfs:label>
    <rdfs:comment>Whether continuous backup recovery is enabled. If not set, defaults to true.</rdfs:comment>
    <rdfs:domain rdf:resource="http://example.org/onto/class/google_alloydb_cluster"/>
    <rdfs:range rdf:resource="http://www.w3.org/2001/XMLSchema#string"/>
  </owl:DatatypeProperty>
  <owl:DatatypeProperty rdf:about="http://example.org/onto/prop/google_alloydb_cluster_recovery_window_days">
    <rdfs:label>recovery_window_days</rdfs:label>
    <rdfs:comment>The numbers of days that are eligible to restore from using PITR. To support the entire recovery window, backups and logs are retained for one day more than the recovery window.

If not set, defaults to 14 days.</rdfs:comment>
    <rdfs:domain rdf:resource="http://example.org/onto/class/google_alloydb_cluster"/>
    <rdfs:range rdf:resource="http://www.w3.org/2001/XMLSchema#string"/>
  </owl:DatatypeProperty>
  <owl:DatatypeProperty rdf:about="http://example.org/onto/prop/google_alloydb_cluster_kms_key_name">
    <rdfs:label>kms_key_name</rdfs:label>
    <rdfs:comment>The fully-qualified resource name of the KMS key. Each Cloud KMS key is regionalized and has the following format: projects/[PROJECT]/locations/[REGION]/keyRings/[RING]/cryptoKeys/[KEY_NAME].</rdfs:comment>
    <rdfs:domain rdf:resource="http://example.org/onto/class/google_alloydb_cluster"/>
    <rdfs:range rdf:resource="http://www.w3.org/2001/XMLSchema#string"/>
  </owl:DatatypeProperty>
  <owl:DatatypeProperty rdf:about="http://example.org/onto/prop/google_alloydb_cluster_kms_key_name">
    <rdfs:label>kms_key_name</rdfs:label>
    <rdfs:comment>The fully-qualified resource name of the KMS key. Each Cloud KMS key is regionalized and has the following format: projects/[PROJECT]/locations/[REGION]/keyRings/[RING]/cryptoKeys/[KEY_NAME].</rdfs:comment>
    <rdfs:domain rdf:resource="http://example.org/onto/class/google_alloydb_cluster"/>
    <rdfs:range rdf:resource="http://www.w3.org/2001/XMLSchema#string"/>
  </owl:DatatypeProperty>
  <owl:DatatypeProperty rdf:about="http://example.org/onto/prop/google_alloydb_cluster_password">
    <rdfs:label>password</rdfs:label>
    <rdfs:comment>The initial password for the user.</rdfs:comment>
    <rdfs:domain rdf:resource="http://example.org/onto/class/google_alloydb_cluster"/>
    <rdfs:range rdf:resource="http://www.w3.org/2001/XMLSchema#string"/>
  </owl:DatatypeProperty>
  <owl:DatatypeProperty rdf:about="http://example.org/onto/prop/google_alloydb_cluster_user">
    <rdfs:label>user</rdfs:label>
    <rdfs:comment>The database username.</rdfs:comment>
    <rdfs:domain rdf:resource="http://example.org/onto/class/google_alloydb_cluster"/>
    <rdfs:range rdf:resource="http://www.w3.org/2001/XMLSchema#string"/>
  </owl:DatatypeProperty>
  <owl:DatatypeProperty rdf:about="http://example.org/onto/prop/google_alloydb_cluster_day">
    <rdfs:label>day</rdfs:label>
    <rdfs:comment>Preferred day of the week for maintenance, e.g. MONDAY, TUESDAY, etc. Possible values: ["MONDAY", "TUESDAY", "WEDNESDAY", "THURSDAY", "FRIDAY", "SATURDAY", "SUNDAY"]</rdfs:comment>
    <rdfs:domain rdf:resource="http://example.org/onto/class/google_alloydb_cluster"/>
    <rdfs:range rdf:resource="http://www.w3.org/2001/XMLSchema#string"/>
  </owl:DatatypeProperty>
  <owl:DatatypeProperty rdf:about="http://example.org/onto/prop/google_alloydb_cluster_hours">
    <rdfs:label>hours</rdfs:label>
    <rdfs:comment>Hours of day in 24 hour format. Should be from 0 to 23.</rdfs:comment>
    <rdfs:domain rdf:resource="http://example.org/onto/class/google_alloydb_cluster"/>
    <rdfs:range rdf:resource="http://www.w3.org/2001/XMLSchema#string"/>
  </owl:DatatypeProperty>
  <owl:DatatypeProperty rdf:about="http://example.org/onto/prop/google_alloydb_cluster_minutes">
    <rdfs:label>minutes</rdfs:label>
    <rdfs:comment>Minutes of hour of day. Currently, only the value 0 is supported.</rdfs:comment>
    <rdfs:domain rdf:resource="http://example.org/onto/class/google_alloydb_cluster"/>
    <rdfs:range rdf:resource="http://www.w3.org/2001/XMLSchema#string"/>
  </owl:DatatypeProperty>
  <owl:DatatypeProperty rdf:about="http://example.org/onto/prop/google_alloydb_cluster_nanos">
    <rdfs:label>nanos</rdfs:label>
    <rdfs:comment>Fractions of seconds in nanoseconds. Currently, only the value 0 is supported.</rdfs:comment>
    <rdfs:domain rdf:resource="http://example.org/onto/class/google_alloydb_cluster"/>
    <rdfs:range rdf:resource="http://www.w3.org/2001/XMLSchema#string"/>
  </owl:DatatypeProperty>
  <owl:DatatypeProperty rdf:about="http://example.org/onto/prop/google_alloydb_cluster_seconds">
    <rdfs:label>seconds</rdfs:label>
    <rdfs:comment>Seconds of minutes of the time. Currently, only the value 0 is supported.</rdfs:comment>
    <rdfs:domain rdf:resource="http://example.org/onto/class/google_alloydb_cluster"/>
    <rdfs:range rdf:resource="http://www.w3.org/2001/XMLSchema#string"/>
  </owl:DatatypeProperty>
  <owl:DatatypeProperty rdf:about="http://example.org/onto/prop/google_alloydb_cluster_allocated_ip_range">
    <rdfs:label>allocated_ip_range</rdfs:label>
    <rdfs:comment>The name of the allocated IP range for the private IP AlloyDB cluster. For example: "google-managed-services-default".
If set, the instance IPs for this cluster will be created in the allocated range.</rdfs:comment>
    <rdfs:domain rdf:resource="http://example.org/onto/class/google_alloydb_cluster"/>
    <rdfs:range rdf:resource="http://www.w3.org/2001/XMLSchema#string"/>
  </owl:DatatypeProperty>
  <owl:DatatypeProperty rdf:about="http://example.org/onto/prop/google_alloydb_cluster_network">
    <rdfs:label>network</rdfs:label>
    <rdfs:comment>The resource link for the VPC network in which cluster resources are created and from which they are accessible via Private IP. The network must belong to the same project as the cluster.
It is specified in the form: "projects/{projectNumber}/global/networks/{network_id}".</rdfs:comment>
    <rdfs:domain rdf:resource="http://example.org/onto/class/google_alloydb_cluster"/>
    <rdfs:range rdf:resource="http://www.w3.org/2001/XMLSchema#string"/>
  </owl:DatatypeProperty>
  <owl:DatatypeProperty rdf:about="http://example.org/onto/prop/google_alloydb_cluster_psc_enabled">
    <rdfs:label>psc_enabled</rdfs:label>
    <rdfs:comment>Create an instance that allows connections from Private Service Connect endpoints to the instance.</rdfs:comment>
    <rdfs:domain rdf:resource="http://example.org/onto/class/google_alloydb_cluster"/>
    <rdfs:range rdf:resource="http://www.w3.org/2001/XMLSchema#string"/>
  </owl:DatatypeProperty>
  <owl:DatatypeProperty rdf:about="http://example.org/onto/prop/google_alloydb_cluster_service_owned_project_number">
    <rdfs:label>service_owned_project_number</rdfs:label>
    <rdfs:comment>The project number that needs to be allowlisted on the network attachment to enable outbound connectivity, if the network attachment is configured to ACCEPT_MANUAL connections.
In case the network attachment is configured to ACCEPT_AUTOMATIC, this project number does not need to be allowlisted explicitly.</rdfs:comment>
    <rdfs:domain rdf:resource="http://example.org/onto/class/google_alloydb_cluster"/>
    <rdfs:range rdf:resource="http://www.w3.org/2001/XMLSchema#string"/>
  </owl:DatatypeProperty>
  <owl:DatatypeProperty rdf:about="http://example.org/onto/prop/google_alloydb_cluster_backup_name">
    <rdfs:label>backup_name</rdfs:label>
    <rdfs:comment>The name of the backup that this cluster is restored from.</rdfs:comment>
    <rdfs:domain rdf:resource="http://example.org/onto/class/google_alloydb_cluster"/>
    <rdfs:range rdf:resource="http://www.w3.org/2001/XMLSchema#string"/>
  </owl:DatatypeProperty>
  <owl:DatatypeProperty rdf:about="http://example.org/onto/prop/google_alloydb_cluster_cluster">
    <rdfs:label>cluster</rdfs:label>
    <rdfs:comment>The name of the source cluster that this cluster is restored from.</rdfs:comment>
    <rdfs:domain rdf:resource="http://example.org/onto/class/google_alloydb_cluster"/>
    <rdfs:range rdf:resource="http://www.w3.org/2001/XMLSchema#string"/>
  </owl:DatatypeProperty>
  <owl:DatatypeProperty rdf:about="http://example.org/onto/prop/google_alloydb_cluster_point_in_time">
    <rdfs:label>point_in_time</rdfs:label>
    <rdfs:comment>The point in time that this cluster is restored to, in RFC 3339 format.</rdfs:comment>
    <rdfs:domain rdf:resource="http://example.org/onto/class/google_alloydb_cluster"/>
    <rdfs:range rdf:resource="http://www.w3.org/2001/XMLSchema#string"/>
  </owl:DatatypeProperty>
  <owl:DatatypeProperty rdf:about="http://example.org/onto/prop/google_alloydb_cluster_primary_cluster_name">
    <rdfs:label>primary_cluster_name</rdfs:label>
    <rdfs:comment>Name of the primary cluster must be in the format
'projects/{project}/locations/{location}/clusters/{cluster_id}'</rdfs:comment>
    <rdfs:domain rdf:resource="http://example.org/onto/class/google_alloydb_cluster"/>
    <rdfs:range rdf:resource="http://www.w3.org/2001/XMLSchema#string"/>
  </owl:DatatypeProperty>
  <owl:DatatypeProperty rdf:about="http://example.org/onto/prop/google_alloydb_cluster_create">
    <rdfs:label>create</rdfs:label>
    <rdfs:domain rdf:resource="http://example.org/onto/class/google_alloydb_cluster"/>
    <rdfs:range rdf:resource="http://www.w3.org/2001/XMLSchema#string"/>
  </owl:DatatypeProperty>
  <owl:DatatypeProperty rdf:about="http://example.org/onto/prop/google_alloydb_cluster_delete">
    <rdfs:label>delete</rdfs:label>
    <rdfs:domain rdf:resource="http://example.org/onto/class/google_alloydb_cluster"/>
    <rdfs:range rdf:resource="http://www.w3.org/2001/XMLSchema#string"/>
  </owl:DatatypeProperty>
  <owl:DatatypeProperty rdf:about="http://example.org/onto/prop/google_alloydb_cluster_update">
    <rdfs:label>update</rdfs:label>
    <rdfs:domain rdf:resource="http://example.org/onto/class/google_alloydb_cluster"/>
    <rdfs:range rdf:resource="http://www.w3.org/2001/XMLSchema#string"/>
  </owl:DatatypeProperty>
</rdf:RDF>
