<?xml version="1.0" encoding="UTF-8"?>
<rdf:RDF
  xmlns:rdf="http://www.w3.org/1999/02/22-rdf-syntax-ns#"
  xmlns:rdfs="http://www.w3.org/2000/01/rdf-schema#"
  xmlns:owl="http://www.w3.org/2002/07/owl#"
  xmlns:xsd="http://www.w3.org/2001/XMLSchema#"
  xml:base="http://example.org/onto/">
  <owl:Class rdf:about="http://example.org/onto/class/google_redis_cluster">
    <rdfs:label>google_redis_cluster</rdfs:label>
    <rdfs:comment>#
#     ***     AUTO GENERATED CODE    ***    Type: MMv1     ***
#
# ----------------------------------------------------------------------------
#
#     This code is generated by Magic Modules using the following:
#
#     Configuration: https:#github.com/GoogleCloudPlatform/magic-modules/tree/main/mmv1/products/redis/Cluster.yaml
#     Template:      https:#github.com/GoogleCloudPlatform/magic-modules/tree/main/mmv1/templates/terraform/resource.html.markdown.tmpl
#
#     DO NOT EDIT this file directly. Any changes made to this file will be
#     overwritten during the next generation cycle.
#
# ----------------------------------------------------------------------------
subcategory: "Memorystore (Redis)"
description: |-
  A Google Cloud Redis Cluster instance.
---</rdfs:comment>
  </owl:Class>
  <owl:DatatypeProperty rdf:about="http://example.org/onto/prop/google_redis_cluster_authorization_mode">
    <rdfs:label>authorization_mode</rdfs:label>
    <rdfs:comment>Optional. The authorization mode of the Redis cluster. If not provided, auth feature is disabled for the cluster. Default value: "AUTH_MODE_DISABLED" Possible values: ["AUTH_MODE_UNSPECIFIED", "AUTH_MODE_IAM_AUTH", "AUTH_MODE_DISABLED"]</rdfs:comment>
    <rdfs:domain rdf:resource="http://example.org/onto/class/google_redis_cluster"/>
    <rdfs:range rdf:resource="http://www.w3.org/2001/XMLSchema#string"/>
  </owl:DatatypeProperty>
  <owl:DatatypeProperty rdf:about="http://example.org/onto/prop/google_redis_cluster_backup_collection">
    <rdfs:label>backup_collection</rdfs:label>
    <rdfs:comment>The backup collection full resource name.
Example: projects/{project}/locations/{location}/backupCollections/{collection}</rdfs:comment>
    <rdfs:domain rdf:resource="http://example.org/onto/class/google_redis_cluster"/>
    <rdfs:range rdf:resource="http://www.w3.org/2001/XMLSchema#string"/>
  </owl:DatatypeProperty>
  <owl:DatatypeProperty rdf:about="http://example.org/onto/prop/google_redis_cluster_create_time">
    <rdfs:label>create_time</rdfs:label>
    <rdfs:comment>The timestamp associated with the cluster creation request. A timestamp in
RFC3339 UTC "Zulu" format, with nanosecond resolution and up to nine fractional
digits. Examples: "2014-10-02T15:01:23Z" and "2014-10-02T15:01:23.045123456Z".</rdfs:comment>
    <rdfs:domain rdf:resource="http://example.org/onto/class/google_redis_cluster"/>
    <rdfs:range rdf:resource="http://www.w3.org/2001/XMLSchema#string"/>
  </owl:DatatypeProperty>
  <owl:DatatypeProperty rdf:about="http://example.org/onto/prop/google_redis_cluster_deletion_protection_enabled">
    <rdfs:label>deletion_protection_enabled</rdfs:label>
    <rdfs:comment>Optional. Indicates if the cluster is deletion protected or not.
If the value if set to true, any delete cluster operation will fail.
Default value is true.</rdfs:comment>
    <rdfs:domain rdf:resource="http://example.org/onto/class/google_redis_cluster"/>
    <rdfs:range rdf:resource="http://www.w3.org/2001/XMLSchema#string"/>
  </owl:DatatypeProperty>
  <owl:DatatypeProperty rdf:about="http://example.org/onto/prop/google_redis_cluster_discovery_endpoints">
    <rdfs:label>discovery_endpoints</rdfs:label>
    <rdfs:comment>Output only. Endpoints created on each given network,
for Redis clients to connect to the cluster.
Currently only one endpoint is supported.</rdfs:comment>
    <rdfs:domain rdf:resource="http://example.org/onto/class/google_redis_cluster"/>
    <rdfs:range rdf:resource="http://www.w3.org/2001/XMLSchema#string"/>
  </owl:DatatypeProperty>
  <owl:DatatypeProperty rdf:about="http://example.org/onto/prop/google_redis_cluster_id">
    <rdfs:label>id</rdfs:label>
    <rdfs:domain rdf:resource="http://example.org/onto/class/google_redis_cluster"/>
    <rdfs:range rdf:resource="http://www.w3.org/2001/XMLSchema#string"/>
  </owl:DatatypeProperty>
  <owl:DatatypeProperty rdf:about="http://example.org/onto/prop/google_redis_cluster_kms_key">
    <rdfs:label>kms_key</rdfs:label>
    <rdfs:comment>The KMS key used to encrypt the at-rest data of the cluster.</rdfs:comment>
    <rdfs:domain rdf:resource="http://example.org/onto/class/google_redis_cluster"/>
    <rdfs:range rdf:resource="http://www.w3.org/2001/XMLSchema#string"/>
  </owl:DatatypeProperty>
  <owl:DatatypeProperty rdf:about="http://example.org/onto/prop/google_redis_cluster_maintenance_schedule">
    <rdfs:label>maintenance_schedule</rdfs:label>
    <rdfs:comment>Upcoming maintenance schedule.</rdfs:comment>
    <rdfs:domain rdf:resource="http://example.org/onto/class/google_redis_cluster"/>
    <rdfs:range rdf:resource="http://www.w3.org/2001/XMLSchema#string"/>
  </owl:DatatypeProperty>
  <owl:DatatypeProperty rdf:about="http://example.org/onto/prop/google_redis_cluster_managed_server_ca">
    <rdfs:label>managed_server_ca</rdfs:label>
    <rdfs:comment>Cluster's Certificate Authority. This field will only be populated if Redis Cluster's transit_encryption_mode is TRANSIT_ENCRYPTION_MODE_SERVER_AUTHENTICATION</rdfs:comment>
    <rdfs:domain rdf:resource="http://example.org/onto/class/google_redis_cluster"/>
    <rdfs:range rdf:resource="http://www.w3.org/2001/XMLSchema#string"/>
  </owl:DatatypeProperty>
  <owl:DatatypeProperty rdf:about="http://example.org/onto/prop/google_redis_cluster_name">
    <rdfs:label>name</rdfs:label>
    <rdfs:comment>Unique name of the resource in this scope including project and location using the form:
projects/{projectId}/locations/{locationId}/clusters/{clusterId}</rdfs:comment>
    <rdfs:domain rdf:resource="http://example.org/onto/class/google_redis_cluster"/>
    <rdfs:range rdf:resource="http://www.w3.org/2001/XMLSchema#string"/>
  </owl:DatatypeProperty>
  <owl:DatatypeProperty rdf:about="http://example.org/onto/prop/google_redis_cluster_node_type">
    <rdfs:label>node_type</rdfs:label>
    <rdfs:comment>The nodeType for the Redis cluster.
If not provided, REDIS_HIGHMEM_MEDIUM will be used as default Possible values: ["REDIS_SHARED_CORE_NANO", "REDIS_HIGHMEM_MEDIUM", "REDIS_HIGHMEM_XLARGE", "REDIS_STANDARD_SMALL"]</rdfs:comment>
    <rdfs:domain rdf:resource="http://example.org/onto/class/google_redis_cluster"/>
    <rdfs:range rdf:resource="http://www.w3.org/2001/XMLSchema#string"/>
  </owl:DatatypeProperty>
  <owl:DatatypeProperty rdf:about="http://example.org/onto/prop/google_redis_cluster_precise_size_gb">
    <rdfs:label>precise_size_gb</rdfs:label>
    <rdfs:comment>Output only. Redis memory precise size in GB for the entire cluster.</rdfs:comment>
    <rdfs:domain rdf:resource="http://example.org/onto/class/google_redis_cluster"/>
    <rdfs:range rdf:resource="http://www.w3.org/2001/XMLSchema#string"/>
  </owl:DatatypeProperty>
  <owl:DatatypeProperty rdf:about="http://example.org/onto/prop/google_redis_cluster_project">
    <rdfs:label>project</rdfs:label>
    <rdfs:domain rdf:resource="http://example.org/onto/class/google_redis_cluster"/>
    <rdfs:range rdf:resource="http://www.w3.org/2001/XMLSchema#string"/>
  </owl:DatatypeProperty>
  <owl:DatatypeProperty rdf:about="http://example.org/onto/prop/google_redis_cluster_psc_connections">
    <rdfs:label>psc_connections</rdfs:label>
    <rdfs:comment>Output only. PSC connections for discovery of the cluster topology and accessing the cluster.</rdfs:comment>
    <rdfs:domain rdf:resource="http://example.org/onto/class/google_redis_cluster"/>
    <rdfs:range rdf:resource="http://www.w3.org/2001/XMLSchema#string"/>
  </owl:DatatypeProperty>
  <owl:DatatypeProperty rdf:about="http://example.org/onto/prop/google_redis_cluster_psc_service_attachments">
    <rdfs:label>psc_service_attachments</rdfs:label>
    <rdfs:comment>Service attachment details to configure Psc connections.</rdfs:comment>
    <rdfs:domain rdf:resource="http://example.org/onto/class/google_redis_cluster"/>
    <rdfs:range rdf:resource="http://www.w3.org/2001/XMLSchema#string"/>
  </owl:DatatypeProperty>
  <owl:DatatypeProperty rdf:about="http://example.org/onto/prop/google_redis_cluster_redis_configs">
    <rdfs:label>redis_configs</rdfs:label>
    <rdfs:comment>Configure Redis Cluster behavior using a subset of native Redis configuration parameters.
Please check Memorystore documentation for the list of supported parameters:
https://cloud.google.com/memorystore/docs/cluster/supported-instance-configurations</rdfs:comment>
    <rdfs:domain rdf:resource="http://example.org/onto/class/google_redis_cluster"/>
    <rdfs:range rdf:resource="http://www.w3.org/2001/XMLSchema#string"/>
  </owl:DatatypeProperty>
  <owl:DatatypeProperty rdf:about="http://example.org/onto/prop/google_redis_cluster_region">
    <rdfs:label>region</rdfs:label>
    <rdfs:comment>The name of the region of the Redis cluster.</rdfs:comment>
    <rdfs:domain rdf:resource="http://example.org/onto/class/google_redis_cluster"/>
    <rdfs:range rdf:resource="http://www.w3.org/2001/XMLSchema#string"/>
  </owl:DatatypeProperty>
  <owl:DatatypeProperty rdf:about="http://example.org/onto/prop/google_redis_cluster_replica_count">
    <rdfs:label>replica_count</rdfs:label>
    <rdfs:comment>Optional. The number of replica nodes per shard.</rdfs:comment>
    <rdfs:domain rdf:resource="http://example.org/onto/class/google_redis_cluster"/>
    <rdfs:range rdf:resource="http://www.w3.org/2001/XMLSchema#string"/>
  </owl:DatatypeProperty>
  <owl:DatatypeProperty rdf:about="http://example.org/onto/prop/google_redis_cluster_shard_count">
    <rdfs:label>shard_count</rdfs:label>
    <rdfs:comment>Required. Number of shards for the Redis cluster.</rdfs:comment>
    <rdfs:domain rdf:resource="http://example.org/onto/class/google_redis_cluster"/>
    <rdfs:range rdf:resource="http://www.w3.org/2001/XMLSchema#string"/>
  </owl:DatatypeProperty>
  <owl:DatatypeProperty rdf:about="http://example.org/onto/prop/google_redis_cluster_size_gb">
    <rdfs:label>size_gb</rdfs:label>
    <rdfs:comment>Output only. Redis memory size in GB for the entire cluster.</rdfs:comment>
    <rdfs:domain rdf:resource="http://example.org/onto/class/google_redis_cluster"/>
    <rdfs:range rdf:resource="http://www.w3.org/2001/XMLSchema#string"/>
  </owl:DatatypeProperty>
  <owl:DatatypeProperty rdf:about="http://example.org/onto/prop/google_redis_cluster_state">
    <rdfs:label>state</rdfs:label>
    <rdfs:comment>The current state of this cluster. Can be CREATING, READY, UPDATING, DELETING and SUSPENDED</rdfs:comment>
    <rdfs:domain rdf:resource="http://example.org/onto/class/google_redis_cluster"/>
    <rdfs:range rdf:resource="http://www.w3.org/2001/XMLSchema#string"/>
  </owl:DatatypeProperty>
  <owl:DatatypeProperty rdf:about="http://example.org/onto/prop/google_redis_cluster_state_info">
    <rdfs:label>state_info</rdfs:label>
    <rdfs:comment>Output only. Additional information about the current state of the cluster.</rdfs:comment>
    <rdfs:domain rdf:resource="http://example.org/onto/class/google_redis_cluster"/>
    <rdfs:range rdf:resource="http://www.w3.org/2001/XMLSchema#string"/>
  </owl:DatatypeProperty>
  <owl:DatatypeProperty rdf:about="http://example.org/onto/prop/google_redis_cluster_transit_encryption_mode">
    <rdfs:label>transit_encryption_mode</rdfs:label>
    <rdfs:comment>Optional. The in-transit encryption for the Redis cluster.
If not provided, encryption is disabled for the cluster. Default value: "TRANSIT_ENCRYPTION_MODE_DISABLED" Possible values: ["TRANSIT_ENCRYPTION_MODE_UNSPECIFIED", "TRANSIT_ENCRYPTION_MODE_DISABLED", "TRANSIT_ENCRYPTION_MODE_SERVER_AUTHENTICATION"]</rdfs:comment>
    <rdfs:domain rdf:resource="http://example.org/onto/class/google_redis_cluster"/>
    <rdfs:range rdf:resource="http://www.w3.org/2001/XMLSchema#string"/>
  </owl:DatatypeProperty>
  <owl:DatatypeProperty rdf:about="http://example.org/onto/prop/google_redis_cluster_uid">
    <rdfs:label>uid</rdfs:label>
    <rdfs:comment>System assigned, unique identifier for the cluster.</rdfs:comment>
    <rdfs:domain rdf:resource="http://example.org/onto/class/google_redis_cluster"/>
    <rdfs:range rdf:resource="http://www.w3.org/2001/XMLSchema#string"/>
  </owl:DatatypeProperty>
  <owl:DatatypeProperty rdf:about="http://example.org/onto/prop/google_redis_cluster_retention">
    <rdfs:label>retention</rdfs:label>
    <rdfs:comment>How long to keep automated backups before the backups are deleted.
The value should be between 1 day and 365 days. If not specified, the default value is 35 days.
A duration in seconds with up to nine fractional digits, ending with 's'. Example: "3.5s".</rdfs:comment>
    <rdfs:domain rdf:resource="http://example.org/onto/class/google_redis_cluster"/>
    <rdfs:range rdf:resource="http://www.w3.org/2001/XMLSchema#string"/>
  </owl:DatatypeProperty>
  <owl:DatatypeProperty rdf:about="http://example.org/onto/prop/google_redis_cluster_hours">
    <rdfs:label>hours</rdfs:label>
    <rdfs:comment>Hours of a day in 24 hour format. Must be greater than or equal to 0 and typically must be less than or equal to 23.
An API may choose to allow the value "24:00:00" for scenarios like business closing time.</rdfs:comment>
    <rdfs:domain rdf:resource="http://example.org/onto/class/google_redis_cluster"/>
    <rdfs:range rdf:resource="http://www.w3.org/2001/XMLSchema#string"/>
  </owl:DatatypeProperty>
  <owl:DatatypeProperty rdf:about="http://example.org/onto/prop/google_redis_cluster_cluster_role">
    <rdfs:label>cluster_role</rdfs:label>
    <rdfs:comment>The role of the cluster in cross cluster replication. Supported values are:

1. 'CLUSTER_ROLE_UNSPECIFIED': This is an independent cluster that has never participated in cross cluster replication. It allows both reads and writes.

1. 'NONE': This is an independent cluster that previously participated in cross cluster replication(either as a 'PRIMARY' or 'SECONDARY' cluster). It allows both reads and writes.

1. 'PRIMARY': This cluster serves as the replication source for secondary clusters that are replicating from it. Any data written to it is automatically replicated to its secondary clusters. It allows both reads and writes.

1. 'SECONDARY': This cluster replicates data from the primary cluster. It allows only reads. Possible values: ["CLUSTER_ROLE_UNSPECIFIED", "NONE", "PRIMARY", "SECONDARY"]</rdfs:comment>
    <rdfs:domain rdf:resource="http://example.org/onto/class/google_redis_cluster"/>
    <rdfs:range rdf:resource="http://www.w3.org/2001/XMLSchema#string"/>
  </owl:DatatypeProperty>
  <owl:DatatypeProperty rdf:about="http://example.org/onto/prop/google_redis_cluster_membership">
    <rdfs:label>membership</rdfs:label>
    <rdfs:comment>An output only view of all the member clusters participating in cross cluster replication. This field is populated for all the member clusters irrespective of their cluster role.</rdfs:comment>
    <rdfs:domain rdf:resource="http://example.org/onto/class/google_redis_cluster"/>
    <rdfs:range rdf:resource="http://www.w3.org/2001/XMLSchema#string"/>
  </owl:DatatypeProperty>
  <owl:DatatypeProperty rdf:about="http://example.org/onto/prop/google_redis_cluster_update_time">
    <rdfs:label>update_time</rdfs:label>
    <rdfs:comment>The last time cross cluster replication config was updated.</rdfs:comment>
    <rdfs:domain rdf:resource="http://example.org/onto/class/google_redis_cluster"/>
    <rdfs:range rdf:resource="http://www.w3.org/2001/XMLSchema#string"/>
  </owl:DatatypeProperty>
  <owl:DatatypeProperty rdf:about="http://example.org/onto/prop/google_redis_cluster_cluster">
    <rdfs:label>cluster</rdfs:label>
    <rdfs:comment>The full resource path of the primary cluster in the format: projects/{project}/locations/{region}/clusters/{cluster-id}</rdfs:comment>
    <rdfs:domain rdf:resource="http://example.org/onto/class/google_redis_cluster"/>
    <rdfs:range rdf:resource="http://www.w3.org/2001/XMLSchema#string"/>
  </owl:DatatypeProperty>
  <owl:DatatypeProperty rdf:about="http://example.org/onto/prop/google_redis_cluster_uid">
    <rdfs:label>uid</rdfs:label>
    <rdfs:comment>The unique id of the primary cluster.</rdfs:comment>
    <rdfs:domain rdf:resource="http://example.org/onto/class/google_redis_cluster"/>
    <rdfs:range rdf:resource="http://www.w3.org/2001/XMLSchema#string"/>
  </owl:DatatypeProperty>
  <owl:DatatypeProperty rdf:about="http://example.org/onto/prop/google_redis_cluster_cluster">
    <rdfs:label>cluster</rdfs:label>
    <rdfs:comment>The full resource path of the secondary cluster in the format: projects/{project}/locations/{region}/clusters/{cluster-id}</rdfs:comment>
    <rdfs:domain rdf:resource="http://example.org/onto/class/google_redis_cluster"/>
    <rdfs:range rdf:resource="http://www.w3.org/2001/XMLSchema#string"/>
  </owl:DatatypeProperty>
  <owl:DatatypeProperty rdf:about="http://example.org/onto/prop/google_redis_cluster_uid">
    <rdfs:label>uid</rdfs:label>
    <rdfs:comment>The unique id of the secondary cluster.</rdfs:comment>
    <rdfs:domain rdf:resource="http://example.org/onto/class/google_redis_cluster"/>
    <rdfs:range rdf:resource="http://www.w3.org/2001/XMLSchema#string"/>
  </owl:DatatypeProperty>
  <owl:DatatypeProperty rdf:about="http://example.org/onto/prop/google_redis_cluster_uris">
    <rdfs:label>uris</rdfs:label>
    <rdfs:comment>URIs of the GCS objects to import. Example: gs://bucket1/object1, gs://bucket2/folder2/object2</rdfs:comment>
    <rdfs:domain rdf:resource="http://example.org/onto/class/google_redis_cluster"/>
    <rdfs:range rdf:resource="http://www.w3.org/2001/XMLSchema#string"/>
  </owl:DatatypeProperty>
  <owl:DatatypeProperty rdf:about="http://example.org/onto/prop/google_redis_cluster_create_time">
    <rdfs:label>create_time</rdfs:label>
    <rdfs:comment>Output only. The time when the policy was created.
A timestamp in RFC3339 UTC "Zulu" format, with nanosecond
resolution and up to nine fractional digits.</rdfs:comment>
    <rdfs:domain rdf:resource="http://example.org/onto/class/google_redis_cluster"/>
    <rdfs:range rdf:resource="http://www.w3.org/2001/XMLSchema#string"/>
  </owl:DatatypeProperty>
  <owl:DatatypeProperty rdf:about="http://example.org/onto/prop/google_redis_cluster_update_time">
    <rdfs:label>update_time</rdfs:label>
    <rdfs:comment>Output only. The time when the policy was last updated.
A timestamp in RFC3339 UTC "Zulu" format, with nanosecond
resolution and up to nine fractional digits.</rdfs:comment>
    <rdfs:domain rdf:resource="http://example.org/onto/class/google_redis_cluster"/>
    <rdfs:range rdf:resource="http://www.w3.org/2001/XMLSchema#string"/>
  </owl:DatatypeProperty>
  <owl:DatatypeProperty rdf:about="http://example.org/onto/prop/google_redis_cluster_day">
    <rdfs:label>day</rdfs:label>
    <rdfs:comment>Required. The day of week that maintenance updates occur.

- DAY_OF_WEEK_UNSPECIFIED: The day of the week is unspecified.
- MONDAY: Monday
- TUESDAY: Tuesday
- WEDNESDAY: Wednesday
- THURSDAY: Thursday
- FRIDAY: Friday
- SATURDAY: Saturday
- SUNDAY: Sunday Possible values: ["DAY_OF_WEEK_UNSPECIFIED", "MONDAY", "TUESDAY", "WEDNESDAY", "THURSDAY", "FRIDAY", "SATURDAY", "SUNDAY"]</rdfs:comment>
    <rdfs:domain rdf:resource="http://example.org/onto/class/google_redis_cluster"/>
    <rdfs:range rdf:resource="http://www.w3.org/2001/XMLSchema#string"/>
  </owl:DatatypeProperty>
  <owl:DatatypeProperty rdf:about="http://example.org/onto/prop/google_redis_cluster_duration">
    <rdfs:label>duration</rdfs:label>
    <rdfs:comment>Output only. Duration of the maintenance window.
The current window is fixed at 1 hour.
A duration in seconds with up to nine fractional digits,
terminated by 's'. Example: "3.5s".</rdfs:comment>
    <rdfs:domain rdf:resource="http://example.org/onto/class/google_redis_cluster"/>
    <rdfs:range rdf:resource="http://www.w3.org/2001/XMLSchema#string"/>
  </owl:DatatypeProperty>
  <owl:DatatypeProperty rdf:about="http://example.org/onto/prop/google_redis_cluster_hours">
    <rdfs:label>hours</rdfs:label>
    <rdfs:comment>Hours of day in 24 hour format. Should be from 0 to 23.
An API may choose to allow the value "24:00:00" for scenarios like business closing time.</rdfs:comment>
    <rdfs:domain rdf:resource="http://example.org/onto/class/google_redis_cluster"/>
    <rdfs:range rdf:resource="http://www.w3.org/2001/XMLSchema#string"/>
  </owl:DatatypeProperty>
  <owl:DatatypeProperty rdf:about="http://example.org/onto/prop/google_redis_cluster_minutes">
    <rdfs:label>minutes</rdfs:label>
    <rdfs:comment>Minutes of hour of day. Must be from 0 to 59.</rdfs:comment>
    <rdfs:domain rdf:resource="http://example.org/onto/class/google_redis_cluster"/>
    <rdfs:range rdf:resource="http://www.w3.org/2001/XMLSchema#string"/>
  </owl:DatatypeProperty>
  <owl:DatatypeProperty rdf:about="http://example.org/onto/prop/google_redis_cluster_nanos">
    <rdfs:label>nanos</rdfs:label>
    <rdfs:comment>Fractions of seconds in nanoseconds. Must be from 0 to 999,999,999.</rdfs:comment>
    <rdfs:domain rdf:resource="http://example.org/onto/class/google_redis_cluster"/>
    <rdfs:range rdf:resource="http://www.w3.org/2001/XMLSchema#string"/>
  </owl:DatatypeProperty>
  <owl:DatatypeProperty rdf:about="http://example.org/onto/prop/google_redis_cluster_seconds">
    <rdfs:label>seconds</rdfs:label>
    <rdfs:comment>Seconds of minutes of the time. Must normally be from 0 to 59.
An API may allow the value 60 if it allows leap-seconds.</rdfs:comment>
    <rdfs:domain rdf:resource="http://example.org/onto/class/google_redis_cluster"/>
    <rdfs:range rdf:resource="http://www.w3.org/2001/XMLSchema#string"/>
  </owl:DatatypeProperty>
  <owl:DatatypeProperty rdf:about="http://example.org/onto/prop/google_redis_cluster_backup">
    <rdfs:label>backup</rdfs:label>
    <rdfs:comment>Example: 'projects/{project}/locations/{location}/backupCollections/{collection}/backups/{backup}'.</rdfs:comment>
    <rdfs:domain rdf:resource="http://example.org/onto/class/google_redis_cluster"/>
    <rdfs:range rdf:resource="http://www.w3.org/2001/XMLSchema#string"/>
  </owl:DatatypeProperty>
  <owl:DatatypeProperty rdf:about="http://example.org/onto/prop/google_redis_cluster_mode">
    <rdfs:label>mode</rdfs:label>
    <rdfs:comment>Optional. Controls whether Persistence features are enabled. If not provided, the existing value will be used.

- DISABLED: 	Persistence (both backup and restore) is disabled for the cluster.
- RDB: RDB based Persistence is enabled.
- AOF: AOF based Persistence is enabled. Possible values: ["PERSISTENCE_MODE_UNSPECIFIED", "DISABLED", "RDB", "AOF"]</rdfs:comment>
    <rdfs:domain rdf:resource="http://example.org/onto/class/google_redis_cluster"/>
    <rdfs:range rdf:resource="http://www.w3.org/2001/XMLSchema#string"/>
  </owl:DatatypeProperty>
  <owl:DatatypeProperty rdf:about="http://example.org/onto/prop/google_redis_cluster_append_fsync">
    <rdfs:label>append_fsync</rdfs:label>
    <rdfs:comment>Optional. Available fsync modes.

- NO - Do not explicitly call fsync(). Rely on OS defaults.
- EVERYSEC - Call fsync() once per second in a background thread. A balance between performance and durability.
- ALWAYS - Call fsync() for earch write command. Possible values: ["APPEND_FSYNC_UNSPECIFIED", "NO", "EVERYSEC", "ALWAYS"]</rdfs:comment>
    <rdfs:domain rdf:resource="http://example.org/onto/class/google_redis_cluster"/>
    <rdfs:range rdf:resource="http://www.w3.org/2001/XMLSchema#string"/>
  </owl:DatatypeProperty>
  <owl:DatatypeProperty rdf:about="http://example.org/onto/prop/google_redis_cluster_rdb_snapshot_period">
    <rdfs:label>rdb_snapshot_period</rdfs:label>
    <rdfs:comment>Optional. Available snapshot periods for scheduling.

- ONE_HOUR:	Snapshot every 1 hour.
- SIX_HOURS:	Snapshot every 6 hours.
- TWELVE_HOURS:	Snapshot every 12 hours.
- TWENTY_FOUR_HOURS:	Snapshot every 24 hours. Possible values: ["SNAPSHOT_PERIOD_UNSPECIFIED", "ONE_HOUR", "SIX_HOURS", "TWELVE_HOURS", "TWENTY_FOUR_HOURS"]</rdfs:comment>
    <rdfs:domain rdf:resource="http://example.org/onto/class/google_redis_cluster"/>
    <rdfs:range rdf:resource="http://www.w3.org/2001/XMLSchema#string"/>
  </owl:DatatypeProperty>
  <owl:DatatypeProperty rdf:about="http://example.org/onto/prop/google_redis_cluster_rdb_snapshot_start_time">
    <rdfs:label>rdb_snapshot_start_time</rdfs:label>
    <rdfs:comment>The time that the first snapshot was/will be attempted, and to which
future snapshots will be aligned.
If not provided, the current time will be used.</rdfs:comment>
    <rdfs:domain rdf:resource="http://example.org/onto/class/google_redis_cluster"/>
    <rdfs:range rdf:resource="http://www.w3.org/2001/XMLSchema#string"/>
  </owl:DatatypeProperty>
  <owl:DatatypeProperty rdf:about="http://example.org/onto/prop/google_redis_cluster_network">
    <rdfs:label>network</rdfs:label>
    <rdfs:comment>Required. The consumer network where the network address of
the discovery endpoint will be reserved, in the form of
projects/{network_project_id_or_number}/global/networks/{network_id}.</rdfs:comment>
    <rdfs:domain rdf:resource="http://example.org/onto/class/google_redis_cluster"/>
    <rdfs:range rdf:resource="http://www.w3.org/2001/XMLSchema#string"/>
  </owl:DatatypeProperty>
  <owl:DatatypeProperty rdf:about="http://example.org/onto/prop/google_redis_cluster_create">
    <rdfs:label>create</rdfs:label>
    <rdfs:domain rdf:resource="http://example.org/onto/class/google_redis_cluster"/>
    <rdfs:range rdf:resource="http://www.w3.org/2001/XMLSchema#string"/>
  </owl:DatatypeProperty>
  <owl:DatatypeProperty rdf:about="http://example.org/onto/prop/google_redis_cluster_delete">
    <rdfs:label>delete</rdfs:label>
    <rdfs:domain rdf:resource="http://example.org/onto/class/google_redis_cluster"/>
    <rdfs:range rdf:resource="http://www.w3.org/2001/XMLSchema#string"/>
  </owl:DatatypeProperty>
  <owl:DatatypeProperty rdf:about="http://example.org/onto/prop/google_redis_cluster_update">
    <rdfs:label>update</rdfs:label>
    <rdfs:domain rdf:resource="http://example.org/onto/class/google_redis_cluster"/>
    <rdfs:range rdf:resource="http://www.w3.org/2001/XMLSchema#string"/>
  </owl:DatatypeProperty>
  <owl:DatatypeProperty rdf:about="http://example.org/onto/prop/google_redis_cluster_mode">
    <rdfs:label>mode</rdfs:label>
    <rdfs:comment>Immutable. The mode for zone distribution for Memorystore Redis cluster.
If not provided, MULTI_ZONE will be used as default Possible values: ["MULTI_ZONE", "SINGLE_ZONE"]</rdfs:comment>
    <rdfs:domain rdf:resource="http://example.org/onto/class/google_redis_cluster"/>
    <rdfs:range rdf:resource="http://www.w3.org/2001/XMLSchema#string"/>
  </owl:DatatypeProperty>
  <owl:DatatypeProperty rdf:about="http://example.org/onto/prop/google_redis_cluster_zone">
    <rdfs:label>zone</rdfs:label>
    <rdfs:comment>Immutable. The zone for single zone Memorystore Redis cluster.</rdfs:comment>
    <rdfs:domain rdf:resource="http://example.org/onto/class/google_redis_cluster"/>
    <rdfs:range rdf:resource="http://www.w3.org/2001/XMLSchema#string"/>
  </owl:DatatypeProperty>
</rdf:RDF>
