<?xml version="1.0" encoding="UTF-8"?>
<rdf:RDF
  xmlns:rdf="http://www.w3.org/1999/02/22-rdf-syntax-ns#"
  xmlns:rdfs="http://www.w3.org/2000/01/rdf-schema#"
  xmlns:owl="http://www.w3.org/2002/07/owl#"
  xmlns:xsd="http://www.w3.org/2001/XMLSchema#"
  xml:base="http://example.org/onto/">
  <owl:Class rdf:about="http://example.org/onto/class/google_network_services_http_route">
    <rdfs:label>google_network_services_http_route</rdfs:label>
    <rdfs:comment>#
#     ***     AUTO GENERATED CODE    ***    Type: MMv1     ***
#
# ----------------------------------------------------------------------------
#
#     This code is generated by Magic Modules using the following:
#
#     Configuration: https:#github.com/GoogleCloudPlatform/magic-modules/tree/main/mmv1/products/networkservices/HttpRoute.yaml
#     Template:      https:#github.com/GoogleCloudPlatform/magic-modules/tree/main/mmv1/templates/terraform/resource.html.markdown.tmpl
#
#     DO NOT EDIT this file directly. Any changes made to this file will be
#     overwritten during the next generation cycle.
#
# ----------------------------------------------------------------------------
subcategory: "Network Services"
description: |-
  HttpRoute is the resource defining how HTTP traffic should be routed by a Mesh or Gateway resource.
---</rdfs:comment>
  </owl:Class>
  <owl:DatatypeProperty rdf:about="http://example.org/onto/prop/google_network_services_http_route_create_time">
    <rdfs:label>create_time</rdfs:label>
    <rdfs:comment>Time the HttpRoute was created in UTC.</rdfs:comment>
    <rdfs:domain rdf:resource="http://example.org/onto/class/google_network_services_http_route"/>
    <rdfs:range rdf:resource="http://www.w3.org/2001/XMLSchema#string"/>
  </owl:DatatypeProperty>
  <owl:DatatypeProperty rdf:about="http://example.org/onto/prop/google_network_services_http_route_description">
    <rdfs:label>description</rdfs:label>
    <rdfs:comment>A free-text description of the resource. Max length 1024 characters.</rdfs:comment>
    <rdfs:domain rdf:resource="http://example.org/onto/class/google_network_services_http_route"/>
    <rdfs:range rdf:resource="http://www.w3.org/2001/XMLSchema#string"/>
  </owl:DatatypeProperty>
  <owl:DatatypeProperty rdf:about="http://example.org/onto/prop/google_network_services_http_route_effective_labels">
    <rdfs:label>effective_labels</rdfs:label>
    <rdfs:comment>All of labels (key/value pairs) present on the resource in GCP, including the labels configured through Terraform, other clients and services.</rdfs:comment>
    <rdfs:domain rdf:resource="http://example.org/onto/class/google_network_services_http_route"/>
    <rdfs:range rdf:resource="http://www.w3.org/2001/XMLSchema#string"/>
  </owl:DatatypeProperty>
  <owl:DatatypeProperty rdf:about="http://example.org/onto/prop/google_network_services_http_route_gateways">
    <rdfs:label>gateways</rdfs:label>
    <rdfs:comment>Gateways defines a list of gateways this HttpRoute is attached to, as one of the routing rules to route the requests served by the gateway.
Each gateway reference should match the pattern: projects/*/locations/global/gateways/<gateway_name></rdfs:comment>
    <rdfs:domain rdf:resource="http://example.org/onto/class/google_network_services_http_route"/>
    <rdfs:range rdf:resource="http://www.w3.org/2001/XMLSchema#string"/>
  </owl:DatatypeProperty>
  <owl:DatatypeProperty rdf:about="http://example.org/onto/prop/google_network_services_http_route_hostnames">
    <rdfs:label>hostnames</rdfs:label>
    <rdfs:comment>Set of hosts that should match against the HTTP host header to select a HttpRoute to process the request.</rdfs:comment>
    <rdfs:domain rdf:resource="http://example.org/onto/class/google_network_services_http_route"/>
    <rdfs:range rdf:resource="http://www.w3.org/2001/XMLSchema#string"/>
  </owl:DatatypeProperty>
  <owl:DatatypeProperty rdf:about="http://example.org/onto/prop/google_network_services_http_route_id">
    <rdfs:label>id</rdfs:label>
    <rdfs:domain rdf:resource="http://example.org/onto/class/google_network_services_http_route"/>
    <rdfs:range rdf:resource="http://www.w3.org/2001/XMLSchema#string"/>
  </owl:DatatypeProperty>
  <owl:DatatypeProperty rdf:about="http://example.org/onto/prop/google_network_services_http_route_labels">
    <rdfs:label>labels</rdfs:label>
    <rdfs:comment>Set of label tags associated with the HttpRoute resource.

**Note**: This field is non-authoritative, and will only manage the labels present in your configuration.
Please refer to the field 'effective_labels' for all of the labels present on the resource.</rdfs:comment>
    <rdfs:domain rdf:resource="http://example.org/onto/class/google_network_services_http_route"/>
    <rdfs:range rdf:resource="http://www.w3.org/2001/XMLSchema#string"/>
  </owl:DatatypeProperty>
  <owl:DatatypeProperty rdf:about="http://example.org/onto/prop/google_network_services_http_route_meshes">
    <rdfs:label>meshes</rdfs:label>
    <rdfs:comment>Meshes defines a list of meshes this HttpRoute is attached to, as one of the routing rules to route the requests served by the mesh.
Each mesh reference should match the pattern: projects/*/locations/global/meshes/<mesh_name>.
The attached Mesh should be of a type SIDECAR.</rdfs:comment>
    <rdfs:domain rdf:resource="http://example.org/onto/class/google_network_services_http_route"/>
    <rdfs:range rdf:resource="http://www.w3.org/2001/XMLSchema#string"/>
  </owl:DatatypeProperty>
  <owl:DatatypeProperty rdf:about="http://example.org/onto/prop/google_network_services_http_route_name">
    <rdfs:label>name</rdfs:label>
    <rdfs:comment>Name of the HttpRoute resource.</rdfs:comment>
    <rdfs:domain rdf:resource="http://example.org/onto/class/google_network_services_http_route"/>
    <rdfs:range rdf:resource="http://www.w3.org/2001/XMLSchema#string"/>
  </owl:DatatypeProperty>
  <owl:DatatypeProperty rdf:about="http://example.org/onto/prop/google_network_services_http_route_project">
    <rdfs:label>project</rdfs:label>
    <rdfs:domain rdf:resource="http://example.org/onto/class/google_network_services_http_route"/>
    <rdfs:range rdf:resource="http://www.w3.org/2001/XMLSchema#string"/>
  </owl:DatatypeProperty>
  <owl:DatatypeProperty rdf:about="http://example.org/onto/prop/google_network_services_http_route_self_link">
    <rdfs:label>self_link</rdfs:label>
    <rdfs:comment>Server-defined URL of this resource.</rdfs:comment>
    <rdfs:domain rdf:resource="http://example.org/onto/class/google_network_services_http_route"/>
    <rdfs:range rdf:resource="http://www.w3.org/2001/XMLSchema#string"/>
  </owl:DatatypeProperty>
  <owl:DatatypeProperty rdf:about="http://example.org/onto/prop/google_network_services_http_route_terraform_labels">
    <rdfs:label>terraform_labels</rdfs:label>
    <rdfs:comment>The combination of labels configured directly on the resource
 and default labels configured on the provider.</rdfs:comment>
    <rdfs:domain rdf:resource="http://example.org/onto/class/google_network_services_http_route"/>
    <rdfs:range rdf:resource="http://www.w3.org/2001/XMLSchema#string"/>
  </owl:DatatypeProperty>
  <owl:DatatypeProperty rdf:about="http://example.org/onto/prop/google_network_services_http_route_update_time">
    <rdfs:label>update_time</rdfs:label>
    <rdfs:comment>Time the HttpRoute was updated in UTC.</rdfs:comment>
    <rdfs:domain rdf:resource="http://example.org/onto/class/google_network_services_http_route"/>
    <rdfs:range rdf:resource="http://www.w3.org/2001/XMLSchema#string"/>
  </owl:DatatypeProperty>
  <owl:DatatypeProperty rdf:about="http://example.org/onto/prop/google_network_services_http_route_timeout">
    <rdfs:label>timeout</rdfs:label>
    <rdfs:comment>Specifies the timeout for selected route.</rdfs:comment>
    <rdfs:domain rdf:resource="http://example.org/onto/class/google_network_services_http_route"/>
    <rdfs:range rdf:resource="http://www.w3.org/2001/XMLSchema#string"/>
  </owl:DatatypeProperty>
  <owl:DatatypeProperty rdf:about="http://example.org/onto/prop/google_network_services_http_route_allow_credentials">
    <rdfs:label>allow_credentials</rdfs:label>
    <rdfs:comment>In response to a preflight request, setting this to true indicates that the actual request can include user credentials.</rdfs:comment>
    <rdfs:domain rdf:resource="http://example.org/onto/class/google_network_services_http_route"/>
    <rdfs:range rdf:resource="http://www.w3.org/2001/XMLSchema#string"/>
  </owl:DatatypeProperty>
  <owl:DatatypeProperty rdf:about="http://example.org/onto/prop/google_network_services_http_route_allow_headers">
    <rdfs:label>allow_headers</rdfs:label>
    <rdfs:comment>Specifies the content for Access-Control-Allow-Headers header.</rdfs:comment>
    <rdfs:domain rdf:resource="http://example.org/onto/class/google_network_services_http_route"/>
    <rdfs:range rdf:resource="http://www.w3.org/2001/XMLSchema#string"/>
  </owl:DatatypeProperty>
  <owl:DatatypeProperty rdf:about="http://example.org/onto/prop/google_network_services_http_route_allow_methods">
    <rdfs:label>allow_methods</rdfs:label>
    <rdfs:comment>Specifies the content for Access-Control-Allow-Methods header.</rdfs:comment>
    <rdfs:domain rdf:resource="http://example.org/onto/class/google_network_services_http_route"/>
    <rdfs:range rdf:resource="http://www.w3.org/2001/XMLSchema#string"/>
  </owl:DatatypeProperty>
  <owl:DatatypeProperty rdf:about="http://example.org/onto/prop/google_network_services_http_route_allow_origin_regexes">
    <rdfs:label>allow_origin_regexes</rdfs:label>
    <rdfs:comment>Specifies the regular expression patterns that match allowed origins.</rdfs:comment>
    <rdfs:domain rdf:resource="http://example.org/onto/class/google_network_services_http_route"/>
    <rdfs:range rdf:resource="http://www.w3.org/2001/XMLSchema#string"/>
  </owl:DatatypeProperty>
  <owl:DatatypeProperty rdf:about="http://example.org/onto/prop/google_network_services_http_route_allow_origins">
    <rdfs:label>allow_origins</rdfs:label>
    <rdfs:comment>Specifies the list of origins that will be allowed to do CORS requests.</rdfs:comment>
    <rdfs:domain rdf:resource="http://example.org/onto/class/google_network_services_http_route"/>
    <rdfs:range rdf:resource="http://www.w3.org/2001/XMLSchema#string"/>
  </owl:DatatypeProperty>
  <owl:DatatypeProperty rdf:about="http://example.org/onto/prop/google_network_services_http_route_disabled">
    <rdfs:label>disabled</rdfs:label>
    <rdfs:comment>If true, the CORS policy is disabled. The default value is false, which indicates that the CORS policy is in effect.</rdfs:comment>
    <rdfs:domain rdf:resource="http://example.org/onto/class/google_network_services_http_route"/>
    <rdfs:range rdf:resource="http://www.w3.org/2001/XMLSchema#string"/>
  </owl:DatatypeProperty>
  <owl:DatatypeProperty rdf:about="http://example.org/onto/prop/google_network_services_http_route_expose_headers">
    <rdfs:label>expose_headers</rdfs:label>
    <rdfs:comment>Specifies the content for Access-Control-Expose-Headers header.</rdfs:comment>
    <rdfs:domain rdf:resource="http://example.org/onto/class/google_network_services_http_route"/>
    <rdfs:range rdf:resource="http://www.w3.org/2001/XMLSchema#string"/>
  </owl:DatatypeProperty>
  <owl:DatatypeProperty rdf:about="http://example.org/onto/prop/google_network_services_http_route_max_age">
    <rdfs:label>max_age</rdfs:label>
    <rdfs:comment>Specifies how long result of a preflight request can be cached in seconds.</rdfs:comment>
    <rdfs:domain rdf:resource="http://example.org/onto/class/google_network_services_http_route"/>
    <rdfs:range rdf:resource="http://www.w3.org/2001/XMLSchema#string"/>
  </owl:DatatypeProperty>
  <owl:DatatypeProperty rdf:about="http://example.org/onto/prop/google_network_services_http_route_service_name">
    <rdfs:label>service_name</rdfs:label>
    <rdfs:comment>The URL of a BackendService to route traffic to.</rdfs:comment>
    <rdfs:domain rdf:resource="http://example.org/onto/class/google_network_services_http_route"/>
    <rdfs:range rdf:resource="http://www.w3.org/2001/XMLSchema#string"/>
  </owl:DatatypeProperty>
  <owl:DatatypeProperty rdf:about="http://example.org/onto/prop/google_network_services_http_route_weight">
    <rdfs:label>weight</rdfs:label>
    <rdfs:comment>Specifies the proportion of requests forwarded to the backend referenced by the serviceName field. This is computed as: weight/Sum(weights in this destination list). For non-zero values, there may be some epsilon from the exact proportion defined here depending on the precision an implementation supports.
If only one serviceName is specified and it has a weight greater than 0, 100% of the traffic is forwarded to that backend.
If weights are specified for any one service name, they need to be specified for all of them.
If weights are unspecified for all services, then, traffic is distributed in equal proportions to all of them.</rdfs:comment>
    <rdfs:domain rdf:resource="http://example.org/onto/class/google_network_services_http_route"/>
    <rdfs:range rdf:resource="http://www.w3.org/2001/XMLSchema#string"/>
  </owl:DatatypeProperty>
  <owl:DatatypeProperty rdf:about="http://example.org/onto/prop/google_network_services_http_route_http_status">
    <rdfs:label>http_status</rdfs:label>
    <rdfs:comment>The HTTP status code used to abort the request.</rdfs:comment>
    <rdfs:domain rdf:resource="http://example.org/onto/class/google_network_services_http_route"/>
    <rdfs:range rdf:resource="http://www.w3.org/2001/XMLSchema#string"/>
  </owl:DatatypeProperty>
  <owl:DatatypeProperty rdf:about="http://example.org/onto/prop/google_network_services_http_route_percentage">
    <rdfs:label>percentage</rdfs:label>
    <rdfs:comment>The percentage of traffic which will be aborted.</rdfs:comment>
    <rdfs:domain rdf:resource="http://example.org/onto/class/google_network_services_http_route"/>
    <rdfs:range rdf:resource="http://www.w3.org/2001/XMLSchema#string"/>
  </owl:DatatypeProperty>
  <owl:DatatypeProperty rdf:about="http://example.org/onto/prop/google_network_services_http_route_fixed_delay">
    <rdfs:label>fixed_delay</rdfs:label>
    <rdfs:comment>Specify a fixed delay before forwarding the request.</rdfs:comment>
    <rdfs:domain rdf:resource="http://example.org/onto/class/google_network_services_http_route"/>
    <rdfs:range rdf:resource="http://www.w3.org/2001/XMLSchema#string"/>
  </owl:DatatypeProperty>
  <owl:DatatypeProperty rdf:about="http://example.org/onto/prop/google_network_services_http_route_percentage">
    <rdfs:label>percentage</rdfs:label>
    <rdfs:comment>The percentage of traffic on which delay will be injected.</rdfs:comment>
    <rdfs:domain rdf:resource="http://example.org/onto/class/google_network_services_http_route"/>
    <rdfs:range rdf:resource="http://www.w3.org/2001/XMLSchema#string"/>
  </owl:DatatypeProperty>
  <owl:DatatypeProperty rdf:about="http://example.org/onto/prop/google_network_services_http_route_host_redirect">
    <rdfs:label>host_redirect</rdfs:label>
    <rdfs:comment>The host that will be used in the redirect response instead of the one that was supplied in the request.</rdfs:comment>
    <rdfs:domain rdf:resource="http://example.org/onto/class/google_network_services_http_route"/>
    <rdfs:range rdf:resource="http://www.w3.org/2001/XMLSchema#string"/>
  </owl:DatatypeProperty>
  <owl:DatatypeProperty rdf:about="http://example.org/onto/prop/google_network_services_http_route_https_redirect">
    <rdfs:label>https_redirect</rdfs:label>
    <rdfs:comment>If set to true, the URL scheme in the redirected request is set to https.</rdfs:comment>
    <rdfs:domain rdf:resource="http://example.org/onto/class/google_network_services_http_route"/>
    <rdfs:range rdf:resource="http://www.w3.org/2001/XMLSchema#string"/>
  </owl:DatatypeProperty>
  <owl:DatatypeProperty rdf:about="http://example.org/onto/prop/google_network_services_http_route_path_redirect">
    <rdfs:label>path_redirect</rdfs:label>
    <rdfs:comment>The path that will be used in the redirect response instead of the one that was supplied in the request. pathRedirect can not be supplied together with prefixRedirect. Supply one alone or neither. If neither is supplied, the path of the original request will be used for the redirect.</rdfs:comment>
    <rdfs:domain rdf:resource="http://example.org/onto/class/google_network_services_http_route"/>
    <rdfs:range rdf:resource="http://www.w3.org/2001/XMLSchema#string"/>
  </owl:DatatypeProperty>
  <owl:DatatypeProperty rdf:about="http://example.org/onto/prop/google_network_services_http_route_port_redirect">
    <rdfs:label>port_redirect</rdfs:label>
    <rdfs:comment>The port that will be used in the redirected request instead of the one that was supplied in the request.</rdfs:comment>
    <rdfs:domain rdf:resource="http://example.org/onto/class/google_network_services_http_route"/>
    <rdfs:range rdf:resource="http://www.w3.org/2001/XMLSchema#string"/>
  </owl:DatatypeProperty>
  <owl:DatatypeProperty rdf:about="http://example.org/onto/prop/google_network_services_http_route_prefix_rewrite">
    <rdfs:label>prefix_rewrite</rdfs:label>
    <rdfs:comment>Indicates that during redirection, the matched prefix (or path) should be swapped with this value.</rdfs:comment>
    <rdfs:domain rdf:resource="http://example.org/onto/class/google_network_services_http_route"/>
    <rdfs:range rdf:resource="http://www.w3.org/2001/XMLSchema#string"/>
  </owl:DatatypeProperty>
  <owl:DatatypeProperty rdf:about="http://example.org/onto/prop/google_network_services_http_route_response_code">
    <rdfs:label>response_code</rdfs:label>
    <rdfs:comment>The HTTP Status code to use for the redirect.</rdfs:comment>
    <rdfs:domain rdf:resource="http://example.org/onto/class/google_network_services_http_route"/>
    <rdfs:range rdf:resource="http://www.w3.org/2001/XMLSchema#string"/>
  </owl:DatatypeProperty>
  <owl:DatatypeProperty rdf:about="http://example.org/onto/prop/google_network_services_http_route_strip_query">
    <rdfs:label>strip_query</rdfs:label>
    <rdfs:comment>If set to true, any accompanying query portion of the original URL is removed prior to redirecting the request.</rdfs:comment>
    <rdfs:domain rdf:resource="http://example.org/onto/class/google_network_services_http_route"/>
    <rdfs:range rdf:resource="http://www.w3.org/2001/XMLSchema#string"/>
  </owl:DatatypeProperty>
  <owl:DatatypeProperty rdf:about="http://example.org/onto/prop/google_network_services_http_route_add">
    <rdfs:label>add</rdfs:label>
    <rdfs:comment>Add the headers with given map where key is the name of the header, value is the value of the header.</rdfs:comment>
    <rdfs:domain rdf:resource="http://example.org/onto/class/google_network_services_http_route"/>
    <rdfs:range rdf:resource="http://www.w3.org/2001/XMLSchema#string"/>
  </owl:DatatypeProperty>
  <owl:DatatypeProperty rdf:about="http://example.org/onto/prop/google_network_services_http_route_remove">
    <rdfs:label>remove</rdfs:label>
    <rdfs:comment>Remove headers (matching by header names) specified in the list.</rdfs:comment>
    <rdfs:domain rdf:resource="http://example.org/onto/class/google_network_services_http_route"/>
    <rdfs:range rdf:resource="http://www.w3.org/2001/XMLSchema#string"/>
  </owl:DatatypeProperty>
  <owl:DatatypeProperty rdf:about="http://example.org/onto/prop/google_network_services_http_route_set">
    <rdfs:label>set</rdfs:label>
    <rdfs:comment>Completely overwrite/replace the headers with given map where key is the name of the header, value is the value of the header.</rdfs:comment>
    <rdfs:domain rdf:resource="http://example.org/onto/class/google_network_services_http_route"/>
    <rdfs:range rdf:resource="http://www.w3.org/2001/XMLSchema#string"/>
  </owl:DatatypeProperty>
  <owl:DatatypeProperty rdf:about="http://example.org/onto/prop/google_network_services_http_route_service_name">
    <rdfs:label>service_name</rdfs:label>
    <rdfs:comment>The URL of a BackendService to route traffic to.</rdfs:comment>
    <rdfs:domain rdf:resource="http://example.org/onto/class/google_network_services_http_route"/>
    <rdfs:range rdf:resource="http://www.w3.org/2001/XMLSchema#string"/>
  </owl:DatatypeProperty>
  <owl:DatatypeProperty rdf:about="http://example.org/onto/prop/google_network_services_http_route_weight">
    <rdfs:label>weight</rdfs:label>
    <rdfs:comment>Specifies the proportion of requests forwarded to the backend referenced by the serviceName field. This is computed as: weight/Sum(weights in this destination list). For non-zero values, there may be some epsilon from the exact proportion defined here depending on the precision an implementation supports.
If only one serviceName is specified and it has a weight greater than 0, 100% of the traffic is forwarded to that backend.
If weights are specified for any one service name, they need to be specified for all of them.
If weights are unspecified for all services, then, traffic is distributed in equal proportions to all of them.</rdfs:comment>
    <rdfs:domain rdf:resource="http://example.org/onto/class/google_network_services_http_route"/>
    <rdfs:range rdf:resource="http://www.w3.org/2001/XMLSchema#string"/>
  </owl:DatatypeProperty>
  <owl:DatatypeProperty rdf:about="http://example.org/onto/prop/google_network_services_http_route_add">
    <rdfs:label>add</rdfs:label>
    <rdfs:comment>Add the headers with given map where key is the name of the header, value is the value of the header.</rdfs:comment>
    <rdfs:domain rdf:resource="http://example.org/onto/class/google_network_services_http_route"/>
    <rdfs:range rdf:resource="http://www.w3.org/2001/XMLSchema#string"/>
  </owl:DatatypeProperty>
  <owl:DatatypeProperty rdf:about="http://example.org/onto/prop/google_network_services_http_route_remove">
    <rdfs:label>remove</rdfs:label>
    <rdfs:comment>Remove headers (matching by header names) specified in the list.</rdfs:comment>
    <rdfs:domain rdf:resource="http://example.org/onto/class/google_network_services_http_route"/>
    <rdfs:range rdf:resource="http://www.w3.org/2001/XMLSchema#string"/>
  </owl:DatatypeProperty>
  <owl:DatatypeProperty rdf:about="http://example.org/onto/prop/google_network_services_http_route_set">
    <rdfs:label>set</rdfs:label>
    <rdfs:comment>Completely overwrite/replace the headers with given map where key is the name of the header, value is the value of the header.</rdfs:comment>
    <rdfs:domain rdf:resource="http://example.org/onto/class/google_network_services_http_route"/>
    <rdfs:range rdf:resource="http://www.w3.org/2001/XMLSchema#string"/>
  </owl:DatatypeProperty>
  <owl:DatatypeProperty rdf:about="http://example.org/onto/prop/google_network_services_http_route_num_retries">
    <rdfs:label>num_retries</rdfs:label>
    <rdfs:comment>Specifies the allowed number of retries.</rdfs:comment>
    <rdfs:domain rdf:resource="http://example.org/onto/class/google_network_services_http_route"/>
    <rdfs:range rdf:resource="http://www.w3.org/2001/XMLSchema#string"/>
  </owl:DatatypeProperty>
  <owl:DatatypeProperty rdf:about="http://example.org/onto/prop/google_network_services_http_route_per_try_timeout">
    <rdfs:label>per_try_timeout</rdfs:label>
    <rdfs:comment>Specifies a non-zero timeout per retry attempt. A duration in seconds with up to nine fractional digits, ending with 's'. Example: "3.5s".</rdfs:comment>
    <rdfs:domain rdf:resource="http://example.org/onto/class/google_network_services_http_route"/>
    <rdfs:range rdf:resource="http://www.w3.org/2001/XMLSchema#string"/>
  </owl:DatatypeProperty>
  <owl:DatatypeProperty rdf:about="http://example.org/onto/prop/google_network_services_http_route_retry_conditions">
    <rdfs:label>retry_conditions</rdfs:label>
    <rdfs:comment>Specifies one or more conditions when this retry policy applies.</rdfs:comment>
    <rdfs:domain rdf:resource="http://example.org/onto/class/google_network_services_http_route"/>
    <rdfs:range rdf:resource="http://www.w3.org/2001/XMLSchema#string"/>
  </owl:DatatypeProperty>
  <owl:DatatypeProperty rdf:about="http://example.org/onto/prop/google_network_services_http_route_host_rewrite">
    <rdfs:label>host_rewrite</rdfs:label>
    <rdfs:comment>Prior to forwarding the request to the selected destination, the requests host header is replaced by this value.</rdfs:comment>
    <rdfs:domain rdf:resource="http://example.org/onto/class/google_network_services_http_route"/>
    <rdfs:range rdf:resource="http://www.w3.org/2001/XMLSchema#string"/>
  </owl:DatatypeProperty>
  <owl:DatatypeProperty rdf:about="http://example.org/onto/prop/google_network_services_http_route_path_prefix_rewrite">
    <rdfs:label>path_prefix_rewrite</rdfs:label>
    <rdfs:comment>Prior to forwarding the request to the selected destination, the matching portion of the requests path is replaced by this value.</rdfs:comment>
    <rdfs:domain rdf:resource="http://example.org/onto/class/google_network_services_http_route"/>
    <rdfs:range rdf:resource="http://www.w3.org/2001/XMLSchema#string"/>
  </owl:DatatypeProperty>
  <owl:DatatypeProperty rdf:about="http://example.org/onto/prop/google_network_services_http_route_full_path_match">
    <rdfs:label>full_path_match</rdfs:label>
    <rdfs:comment>The HTTP request path value should exactly match this value.</rdfs:comment>
    <rdfs:domain rdf:resource="http://example.org/onto/class/google_network_services_http_route"/>
    <rdfs:range rdf:resource="http://www.w3.org/2001/XMLSchema#string"/>
  </owl:DatatypeProperty>
  <owl:DatatypeProperty rdf:about="http://example.org/onto/prop/google_network_services_http_route_ignore_case">
    <rdfs:label>ignore_case</rdfs:label>
    <rdfs:comment>Specifies if prefixMatch and fullPathMatch matches are case sensitive. The default value is false.</rdfs:comment>
    <rdfs:domain rdf:resource="http://example.org/onto/class/google_network_services_http_route"/>
    <rdfs:range rdf:resource="http://www.w3.org/2001/XMLSchema#string"/>
  </owl:DatatypeProperty>
  <owl:DatatypeProperty rdf:about="http://example.org/onto/prop/google_network_services_http_route_prefix_match">
    <rdfs:label>prefix_match</rdfs:label>
    <rdfs:comment>The HTTP request path value must begin with specified prefixMatch. prefixMatch must begin with a /.</rdfs:comment>
    <rdfs:domain rdf:resource="http://example.org/onto/class/google_network_services_http_route"/>
    <rdfs:range rdf:resource="http://www.w3.org/2001/XMLSchema#string"/>
  </owl:DatatypeProperty>
  <owl:DatatypeProperty rdf:about="http://example.org/onto/prop/google_network_services_http_route_regex_match">
    <rdfs:label>regex_match</rdfs:label>
    <rdfs:comment>The HTTP request path value must satisfy the regular expression specified by regexMatch after removing any query parameters and anchor supplied with the original URL. For regular expression grammar, please see https://github.com/google/re2/wiki/Syntax</rdfs:comment>
    <rdfs:domain rdf:resource="http://example.org/onto/class/google_network_services_http_route"/>
    <rdfs:range rdf:resource="http://www.w3.org/2001/XMLSchema#string"/>
  </owl:DatatypeProperty>
  <owl:DatatypeProperty rdf:about="http://example.org/onto/prop/google_network_services_http_route_exact_match">
    <rdfs:label>exact_match</rdfs:label>
    <rdfs:comment>The value of the header should match exactly the content of exactMatch.</rdfs:comment>
    <rdfs:domain rdf:resource="http://example.org/onto/class/google_network_services_http_route"/>
    <rdfs:range rdf:resource="http://www.w3.org/2001/XMLSchema#string"/>
  </owl:DatatypeProperty>
  <owl:DatatypeProperty rdf:about="http://example.org/onto/prop/google_network_services_http_route_header">
    <rdfs:label>header</rdfs:label>
    <rdfs:comment>The name of the HTTP header to match against.</rdfs:comment>
    <rdfs:domain rdf:resource="http://example.org/onto/class/google_network_services_http_route"/>
    <rdfs:range rdf:resource="http://www.w3.org/2001/XMLSchema#string"/>
  </owl:DatatypeProperty>
  <owl:DatatypeProperty rdf:about="http://example.org/onto/prop/google_network_services_http_route_invert_match">
    <rdfs:label>invert_match</rdfs:label>
    <rdfs:comment>If specified, the match result will be inverted before checking. Default value is set to false.</rdfs:comment>
    <rdfs:domain rdf:resource="http://example.org/onto/class/google_network_services_http_route"/>
    <rdfs:range rdf:resource="http://www.w3.org/2001/XMLSchema#string"/>
  </owl:DatatypeProperty>
  <owl:DatatypeProperty rdf:about="http://example.org/onto/prop/google_network_services_http_route_prefix_match">
    <rdfs:label>prefix_match</rdfs:label>
    <rdfs:comment>The value of the header must start with the contents of prefixMatch.</rdfs:comment>
    <rdfs:domain rdf:resource="http://example.org/onto/class/google_network_services_http_route"/>
    <rdfs:range rdf:resource="http://www.w3.org/2001/XMLSchema#string"/>
  </owl:DatatypeProperty>
  <owl:DatatypeProperty rdf:about="http://example.org/onto/prop/google_network_services_http_route_present_match">
    <rdfs:label>present_match</rdfs:label>
    <rdfs:comment>A header with headerName must exist. The match takes place whether or not the header has a value.</rdfs:comment>
    <rdfs:domain rdf:resource="http://example.org/onto/class/google_network_services_http_route"/>
    <rdfs:range rdf:resource="http://www.w3.org/2001/XMLSchema#string"/>
  </owl:DatatypeProperty>
  <owl:DatatypeProperty rdf:about="http://example.org/onto/prop/google_network_services_http_route_regex_match">
    <rdfs:label>regex_match</rdfs:label>
    <rdfs:comment>The value of the header must match the regular expression specified in regexMatch.</rdfs:comment>
    <rdfs:domain rdf:resource="http://example.org/onto/class/google_network_services_http_route"/>
    <rdfs:range rdf:resource="http://www.w3.org/2001/XMLSchema#string"/>
  </owl:DatatypeProperty>
  <owl:DatatypeProperty rdf:about="http://example.org/onto/prop/google_network_services_http_route_suffix_match">
    <rdfs:label>suffix_match</rdfs:label>
    <rdfs:comment>The value of the header must end with the contents of suffixMatch.</rdfs:comment>
    <rdfs:domain rdf:resource="http://example.org/onto/class/google_network_services_http_route"/>
    <rdfs:range rdf:resource="http://www.w3.org/2001/XMLSchema#string"/>
  </owl:DatatypeProperty>
  <owl:DatatypeProperty rdf:about="http://example.org/onto/prop/google_network_services_http_route_end">
    <rdfs:label>end</rdfs:label>
    <rdfs:comment>End of the range (exclusive).</rdfs:comment>
    <rdfs:domain rdf:resource="http://example.org/onto/class/google_network_services_http_route"/>
    <rdfs:range rdf:resource="http://www.w3.org/2001/XMLSchema#string"/>
  </owl:DatatypeProperty>
  <owl:DatatypeProperty rdf:about="http://example.org/onto/prop/google_network_services_http_route_start">
    <rdfs:label>start</rdfs:label>
    <rdfs:comment>Start of the range (inclusive).</rdfs:comment>
    <rdfs:domain rdf:resource="http://example.org/onto/class/google_network_services_http_route"/>
    <rdfs:range rdf:resource="http://www.w3.org/2001/XMLSchema#string"/>
  </owl:DatatypeProperty>
  <owl:DatatypeProperty rdf:about="http://example.org/onto/prop/google_network_services_http_route_exact_match">
    <rdfs:label>exact_match</rdfs:label>
    <rdfs:comment>The value of the query parameter must exactly match the contents of exactMatch.</rdfs:comment>
    <rdfs:domain rdf:resource="http://example.org/onto/class/google_network_services_http_route"/>
    <rdfs:range rdf:resource="http://www.w3.org/2001/XMLSchema#string"/>
  </owl:DatatypeProperty>
  <owl:DatatypeProperty rdf:about="http://example.org/onto/prop/google_network_services_http_route_present_match">
    <rdfs:label>present_match</rdfs:label>
    <rdfs:comment>Specifies that the QueryParameterMatcher matches if request contains query parameter, irrespective of whether the parameter has a value or not.</rdfs:comment>
    <rdfs:domain rdf:resource="http://example.org/onto/class/google_network_services_http_route"/>
    <rdfs:range rdf:resource="http://www.w3.org/2001/XMLSchema#string"/>
  </owl:DatatypeProperty>
  <owl:DatatypeProperty rdf:about="http://example.org/onto/prop/google_network_services_http_route_query_parameter">
    <rdfs:label>query_parameter</rdfs:label>
    <rdfs:comment>The name of the query parameter to match.</rdfs:comment>
    <rdfs:domain rdf:resource="http://example.org/onto/class/google_network_services_http_route"/>
    <rdfs:range rdf:resource="http://www.w3.org/2001/XMLSchema#string"/>
  </owl:DatatypeProperty>
  <owl:DatatypeProperty rdf:about="http://example.org/onto/prop/google_network_services_http_route_regex_match">
    <rdfs:label>regex_match</rdfs:label>
    <rdfs:comment>The value of the query parameter must match the regular expression specified by regexMatch.For regular expression grammar, please see https://github.com/google/re2/wiki/Syntax</rdfs:comment>
    <rdfs:domain rdf:resource="http://example.org/onto/class/google_network_services_http_route"/>
    <rdfs:range rdf:resource="http://www.w3.org/2001/XMLSchema#string"/>
  </owl:DatatypeProperty>
  <owl:DatatypeProperty rdf:about="http://example.org/onto/prop/google_network_services_http_route_create">
    <rdfs:label>create</rdfs:label>
    <rdfs:domain rdf:resource="http://example.org/onto/class/google_network_services_http_route"/>
    <rdfs:range rdf:resource="http://www.w3.org/2001/XMLSchema#string"/>
  </owl:DatatypeProperty>
  <owl:DatatypeProperty rdf:about="http://example.org/onto/prop/google_network_services_http_route_delete">
    <rdfs:label>delete</rdfs:label>
    <rdfs:domain rdf:resource="http://example.org/onto/class/google_network_services_http_route"/>
    <rdfs:range rdf:resource="http://www.w3.org/2001/XMLSchema#string"/>
  </owl:DatatypeProperty>
  <owl:DatatypeProperty rdf:about="http://example.org/onto/prop/google_network_services_http_route_update">
    <rdfs:label>update</rdfs:label>
    <rdfs:domain rdf:resource="http://example.org/onto/class/google_network_services_http_route"/>
    <rdfs:range rdf:resource="http://www.w3.org/2001/XMLSchema#string"/>
  </owl:DatatypeProperty>
</rdf:RDF>
