<?xml version="1.0" encoding="UTF-8"?>
<rdf:RDF
  xmlns:rdf="http://www.w3.org/1999/02/22-rdf-syntax-ns#"
  xmlns:rdfs="http://www.w3.org/2000/01/rdf-schema#"
  xmlns:owl="http://www.w3.org/2002/07/owl#"
  xmlns:xsd="http://www.w3.org/2001/XMLSchema#"
  xml:base="http://example.org/onto/">
  <owl:Class rdf:about="http://example.org/onto/class/google_dialogflow_cx_webhook">
    <rdfs:label>google_dialogflow_cx_webhook</rdfs:label>
    <rdfs:comment>#
#     ***     AUTO GENERATED CODE    ***    Type: MMv1     ***
#
# ----------------------------------------------------------------------------
#
#     This code is generated by Magic Modules using the following:
#
#     Configuration: https:#github.com/GoogleCloudPlatform/magic-modules/tree/main/mmv1/products/dialogflowcx/Webhook.yaml
#     Template:      https:#github.com/GoogleCloudPlatform/magic-modules/tree/main/mmv1/templates/terraform/resource.html.markdown.tmpl
#
#     DO NOT EDIT this file directly. Any changes made to this file will be
#     overwritten during the next generation cycle.
#
# ----------------------------------------------------------------------------
subcategory: "Dialogflow CX"
description: |-
  Webhooks host the developer's business logic.
---</rdfs:comment>
  </owl:Class>
  <owl:DatatypeProperty rdf:about="http://example.org/onto/prop/google_dialogflow_cx_webhook_disabled">
    <rdfs:label>disabled</rdfs:label>
    <rdfs:comment>Indicates whether the webhook is disabled.</rdfs:comment>
    <rdfs:domain rdf:resource="http://example.org/onto/class/google_dialogflow_cx_webhook"/>
    <rdfs:range rdf:resource="http://www.w3.org/2001/XMLSchema#string"/>
  </owl:DatatypeProperty>
  <owl:DatatypeProperty rdf:about="http://example.org/onto/prop/google_dialogflow_cx_webhook_display_name">
    <rdfs:label>display_name</rdfs:label>
    <rdfs:comment>The human-readable name of the webhook, unique within the agent.</rdfs:comment>
    <rdfs:domain rdf:resource="http://example.org/onto/class/google_dialogflow_cx_webhook"/>
    <rdfs:range rdf:resource="http://www.w3.org/2001/XMLSchema#string"/>
  </owl:DatatypeProperty>
  <owl:DatatypeProperty rdf:about="http://example.org/onto/prop/google_dialogflow_cx_webhook_enable_spell_correction">
    <rdfs:label>enable_spell_correction</rdfs:label>
    <rdfs:comment>Deprecated. Indicates if automatic spell correction is enabled in detect intent requests.</rdfs:comment>
    <rdfs:domain rdf:resource="http://example.org/onto/class/google_dialogflow_cx_webhook"/>
    <rdfs:range rdf:resource="http://www.w3.org/2001/XMLSchema#string"/>
  </owl:DatatypeProperty>
  <owl:DatatypeProperty rdf:about="http://example.org/onto/prop/google_dialogflow_cx_webhook_enable_stackdriver_logging">
    <rdfs:label>enable_stackdriver_logging</rdfs:label>
    <rdfs:comment>Deprecated. Determines whether this agent should log conversation queries.</rdfs:comment>
    <rdfs:domain rdf:resource="http://example.org/onto/class/google_dialogflow_cx_webhook"/>
    <rdfs:range rdf:resource="http://www.w3.org/2001/XMLSchema#string"/>
  </owl:DatatypeProperty>
  <owl:DatatypeProperty rdf:about="http://example.org/onto/prop/google_dialogflow_cx_webhook_id">
    <rdfs:label>id</rdfs:label>
    <rdfs:domain rdf:resource="http://example.org/onto/class/google_dialogflow_cx_webhook"/>
    <rdfs:range rdf:resource="http://www.w3.org/2001/XMLSchema#string"/>
  </owl:DatatypeProperty>
  <owl:DatatypeProperty rdf:about="http://example.org/onto/prop/google_dialogflow_cx_webhook_name">
    <rdfs:label>name</rdfs:label>
    <rdfs:comment>The unique identifier of the webhook.
Format: projects/<Project ID>/locations/<Location ID>/agents/<Agent ID>/webhooks/<Webhook ID>.</rdfs:comment>
    <rdfs:domain rdf:resource="http://example.org/onto/class/google_dialogflow_cx_webhook"/>
    <rdfs:range rdf:resource="http://www.w3.org/2001/XMLSchema#string"/>
  </owl:DatatypeProperty>
  <owl:DatatypeProperty rdf:about="http://example.org/onto/prop/google_dialogflow_cx_webhook_parent">
    <rdfs:label>parent</rdfs:label>
    <rdfs:comment>The agent to create a webhook for.
Format: projects/<Project ID>/locations/<Location ID>/agents/<Agent ID>.</rdfs:comment>
    <rdfs:domain rdf:resource="http://example.org/onto/class/google_dialogflow_cx_webhook"/>
    <rdfs:range rdf:resource="http://www.w3.org/2001/XMLSchema#string"/>
  </owl:DatatypeProperty>
  <owl:DatatypeProperty rdf:about="http://example.org/onto/prop/google_dialogflow_cx_webhook_security_settings">
    <rdfs:label>security_settings</rdfs:label>
    <rdfs:comment>Deprecated. Name of the SecuritySettings reference for the agent. Format: projects/<Project ID>/locations/<Location ID>/securitySettings/<Security Settings ID>.</rdfs:comment>
    <rdfs:domain rdf:resource="http://example.org/onto/class/google_dialogflow_cx_webhook"/>
    <rdfs:range rdf:resource="http://www.w3.org/2001/XMLSchema#string"/>
  </owl:DatatypeProperty>
  <owl:DatatypeProperty rdf:about="http://example.org/onto/prop/google_dialogflow_cx_webhook_start_flow">
    <rdfs:label>start_flow</rdfs:label>
    <rdfs:comment>Deprecated. Name of the start flow in this agent. A start flow will be automatically created when the agent is created, and can only be deleted by deleting the agent. Format: projects/<Project ID>/locations/<Location ID>/agents/<Agent ID>/flows/<Flow ID>.</rdfs:comment>
    <rdfs:domain rdf:resource="http://example.org/onto/class/google_dialogflow_cx_webhook"/>
    <rdfs:range rdf:resource="http://www.w3.org/2001/XMLSchema#string"/>
  </owl:DatatypeProperty>
  <owl:DatatypeProperty rdf:about="http://example.org/onto/prop/google_dialogflow_cx_webhook_timeout">
    <rdfs:label>timeout</rdfs:label>
    <rdfs:comment>Webhook execution timeout.</rdfs:comment>
    <rdfs:domain rdf:resource="http://example.org/onto/class/google_dialogflow_cx_webhook"/>
    <rdfs:range rdf:resource="http://www.w3.org/2001/XMLSchema#string"/>
  </owl:DatatypeProperty>
  <owl:DatatypeProperty rdf:about="http://example.org/onto/prop/google_dialogflow_cx_webhook_allowed_ca_certs">
    <rdfs:label>allowed_ca_certs</rdfs:label>
    <rdfs:comment>Specifies a list of allowed custom CA certificates (in DER format) for
HTTPS verification. This overrides the default SSL trust store. If this
is empty or unspecified, Dialogflow will use Google's default trust store
to verify certificates.
N.B. Make sure the HTTPS server certificates are signed with "subject alt
name". For instance a certificate can be self-signed using the following
command,
openssl x509 -req -days 200 -in example.com.csr \
-signkey example.com.key \
-out example.com.crt \
-extfile <(printf "\nsubjectAltName='DNS:www.example.com'")</rdfs:comment>
    <rdfs:domain rdf:resource="http://example.org/onto/class/google_dialogflow_cx_webhook"/>
    <rdfs:range rdf:resource="http://www.w3.org/2001/XMLSchema#string"/>
  </owl:DatatypeProperty>
  <owl:DatatypeProperty rdf:about="http://example.org/onto/prop/google_dialogflow_cx_webhook_http_method">
    <rdfs:label>http_method</rdfs:label>
    <rdfs:comment>HTTP method for the flexible webhook calls. Standard webhook always uses
POST. Possible values: ["POST", "GET", "HEAD", "PUT", "DELETE", "PATCH", "OPTIONS"]</rdfs:comment>
    <rdfs:domain rdf:resource="http://example.org/onto/class/google_dialogflow_cx_webhook"/>
    <rdfs:range rdf:resource="http://www.w3.org/2001/XMLSchema#string"/>
  </owl:DatatypeProperty>
  <owl:DatatypeProperty rdf:about="http://example.org/onto/prop/google_dialogflow_cx_webhook_parameter_mapping">
    <rdfs:label>parameter_mapping</rdfs:label>
    <rdfs:comment>Maps the values extracted from specific fields of the flexible webhook
response into session parameters.
- Key: session parameter name
- Value: field path in the webhook response</rdfs:comment>
    <rdfs:domain rdf:resource="http://example.org/onto/class/google_dialogflow_cx_webhook"/>
    <rdfs:range rdf:resource="http://www.w3.org/2001/XMLSchema#string"/>
  </owl:DatatypeProperty>
  <owl:DatatypeProperty rdf:about="http://example.org/onto/prop/google_dialogflow_cx_webhook_request_body">
    <rdfs:label>request_body</rdfs:label>
    <rdfs:comment>Defines a custom JSON object as request body to send to flexible webhook.</rdfs:comment>
    <rdfs:domain rdf:resource="http://example.org/onto/class/google_dialogflow_cx_webhook"/>
    <rdfs:range rdf:resource="http://www.w3.org/2001/XMLSchema#string"/>
  </owl:DatatypeProperty>
  <owl:DatatypeProperty rdf:about="http://example.org/onto/prop/google_dialogflow_cx_webhook_request_headers">
    <rdfs:label>request_headers</rdfs:label>
    <rdfs:comment>The HTTP request headers to send together with webhook requests.</rdfs:comment>
    <rdfs:domain rdf:resource="http://example.org/onto/class/google_dialogflow_cx_webhook"/>
    <rdfs:range rdf:resource="http://www.w3.org/2001/XMLSchema#string"/>
  </owl:DatatypeProperty>
  <owl:DatatypeProperty rdf:about="http://example.org/onto/prop/google_dialogflow_cx_webhook_secret_version_for_username_password">
    <rdfs:label>secret_version_for_username_password</rdfs:label>
    <rdfs:comment>The SecretManager secret version resource storing the username:password
pair for HTTP Basic authentication.
Format: 'projects/{project}/secrets/{secret}/versions/{version}'</rdfs:comment>
    <rdfs:domain rdf:resource="http://example.org/onto/class/google_dialogflow_cx_webhook"/>
    <rdfs:range rdf:resource="http://www.w3.org/2001/XMLSchema#string"/>
  </owl:DatatypeProperty>
  <owl:DatatypeProperty rdf:about="http://example.org/onto/prop/google_dialogflow_cx_webhook_service_agent_auth">
    <rdfs:label>service_agent_auth</rdfs:label>
    <rdfs:comment>Indicate the auth token type generated from the [Diglogflow service
agent](https://cloud.google.com/iam/docs/service-agents#dialogflow-service-agent).
The generated token is sent in the Authorization header. Possible values: ["NONE", "ID_TOKEN", "ACCESS_TOKEN"]</rdfs:comment>
    <rdfs:domain rdf:resource="http://example.org/onto/class/google_dialogflow_cx_webhook"/>
    <rdfs:range rdf:resource="http://www.w3.org/2001/XMLSchema#string"/>
  </owl:DatatypeProperty>
  <owl:DatatypeProperty rdf:about="http://example.org/onto/prop/google_dialogflow_cx_webhook_uri">
    <rdfs:label>uri</rdfs:label>
    <rdfs:comment>The webhook URI for receiving POST requests. It must use https protocol.</rdfs:comment>
    <rdfs:domain rdf:resource="http://example.org/onto/class/google_dialogflow_cx_webhook"/>
    <rdfs:range rdf:resource="http://www.w3.org/2001/XMLSchema#string"/>
  </owl:DatatypeProperty>
  <owl:DatatypeProperty rdf:about="http://example.org/onto/prop/google_dialogflow_cx_webhook_webhook_type">
    <rdfs:label>webhook_type</rdfs:label>
    <rdfs:comment>Type of the webhook. Possible values: ["STANDARD", "FLEXIBLE"]</rdfs:comment>
    <rdfs:domain rdf:resource="http://example.org/onto/class/google_dialogflow_cx_webhook"/>
    <rdfs:range rdf:resource="http://www.w3.org/2001/XMLSchema#string"/>
  </owl:DatatypeProperty>
  <owl:DatatypeProperty rdf:about="http://example.org/onto/prop/google_dialogflow_cx_webhook_client_id">
    <rdfs:label>client_id</rdfs:label>
    <rdfs:comment>The client ID provided by the 3rd party platform.</rdfs:comment>
    <rdfs:domain rdf:resource="http://example.org/onto/class/google_dialogflow_cx_webhook"/>
    <rdfs:range rdf:resource="http://www.w3.org/2001/XMLSchema#string"/>
  </owl:DatatypeProperty>
  <owl:DatatypeProperty rdf:about="http://example.org/onto/prop/google_dialogflow_cx_webhook_client_secret">
    <rdfs:label>client_secret</rdfs:label>
    <rdfs:comment>The client secret provided by the 3rd party platform.  If the
'secret_version_for_client_secret' field is set, this field will be
ignored.</rdfs:comment>
    <rdfs:domain rdf:resource="http://example.org/onto/class/google_dialogflow_cx_webhook"/>
    <rdfs:range rdf:resource="http://www.w3.org/2001/XMLSchema#string"/>
  </owl:DatatypeProperty>
  <owl:DatatypeProperty rdf:about="http://example.org/onto/prop/google_dialogflow_cx_webhook_scopes">
    <rdfs:label>scopes</rdfs:label>
    <rdfs:comment>The OAuth scopes to grant.</rdfs:comment>
    <rdfs:domain rdf:resource="http://example.org/onto/class/google_dialogflow_cx_webhook"/>
    <rdfs:range rdf:resource="http://www.w3.org/2001/XMLSchema#string"/>
  </owl:DatatypeProperty>
  <owl:DatatypeProperty rdf:about="http://example.org/onto/prop/google_dialogflow_cx_webhook_secret_version_for_client_secret">
    <rdfs:label>secret_version_for_client_secret</rdfs:label>
    <rdfs:comment>The name of the SecretManager secret version resource storing the
client secret. If this field is set, the 'client_secret' field will be
ignored.
Format: 'projects/{project}/secrets/{secret}/versions/{version}'</rdfs:comment>
    <rdfs:domain rdf:resource="http://example.org/onto/class/google_dialogflow_cx_webhook"/>
    <rdfs:range rdf:resource="http://www.w3.org/2001/XMLSchema#string"/>
  </owl:DatatypeProperty>
  <owl:DatatypeProperty rdf:about="http://example.org/onto/prop/google_dialogflow_cx_webhook_token_endpoint">
    <rdfs:label>token_endpoint</rdfs:label>
    <rdfs:comment>The token endpoint provided by the 3rd party platform to exchange an
access token.</rdfs:comment>
    <rdfs:domain rdf:resource="http://example.org/onto/class/google_dialogflow_cx_webhook"/>
    <rdfs:range rdf:resource="http://www.w3.org/2001/XMLSchema#string"/>
  </owl:DatatypeProperty>
  <owl:DatatypeProperty rdf:about="http://example.org/onto/prop/google_dialogflow_cx_webhook_key">
    <rdfs:label>key</rdfs:label>
    <rdfs:domain rdf:resource="http://example.org/onto/class/google_dialogflow_cx_webhook"/>
    <rdfs:range rdf:resource="http://www.w3.org/2001/XMLSchema#string"/>
  </owl:DatatypeProperty>
  <owl:DatatypeProperty rdf:about="http://example.org/onto/prop/google_dialogflow_cx_webhook_secret_version">
    <rdfs:label>secret_version</rdfs:label>
    <rdfs:comment>The SecretManager secret version resource storing the header value.
Format: 'projects/{project}/secrets/{secret}/versions/{version}'</rdfs:comment>
    <rdfs:domain rdf:resource="http://example.org/onto/class/google_dialogflow_cx_webhook"/>
    <rdfs:range rdf:resource="http://www.w3.org/2001/XMLSchema#string"/>
  </owl:DatatypeProperty>
  <owl:DatatypeProperty rdf:about="http://example.org/onto/prop/google_dialogflow_cx_webhook_service">
    <rdfs:label>service</rdfs:label>
    <rdfs:comment>The name of Service Directory service.</rdfs:comment>
    <rdfs:domain rdf:resource="http://example.org/onto/class/google_dialogflow_cx_webhook"/>
    <rdfs:range rdf:resource="http://www.w3.org/2001/XMLSchema#string"/>
  </owl:DatatypeProperty>
  <owl:DatatypeProperty rdf:about="http://example.org/onto/prop/google_dialogflow_cx_webhook_allowed_ca_certs">
    <rdfs:label>allowed_ca_certs</rdfs:label>
    <rdfs:comment>Specifies a list of allowed custom CA certificates (in DER format) for
HTTPS verification. This overrides the default SSL trust store. If this
is empty or unspecified, Dialogflow will use Google's default trust store
to verify certificates.
N.B. Make sure the HTTPS server certificates are signed with "subject alt
name". For instance a certificate can be self-signed using the following
command,
openssl x509 -req -days 200 -in example.com.csr \
-signkey example.com.key \
-out example.com.crt \
-extfile <(printf "\nsubjectAltName='DNS:www.example.com'")</rdfs:comment>
    <rdfs:domain rdf:resource="http://example.org/onto/class/google_dialogflow_cx_webhook"/>
    <rdfs:range rdf:resource="http://www.w3.org/2001/XMLSchema#string"/>
  </owl:DatatypeProperty>
  <owl:DatatypeProperty rdf:about="http://example.org/onto/prop/google_dialogflow_cx_webhook_http_method">
    <rdfs:label>http_method</rdfs:label>
    <rdfs:comment>HTTP method for the flexible webhook calls. Standard webhook always uses
POST. Possible values: ["POST", "GET", "HEAD", "PUT", "DELETE", "PATCH", "OPTIONS"]</rdfs:comment>
    <rdfs:domain rdf:resource="http://example.org/onto/class/google_dialogflow_cx_webhook"/>
    <rdfs:range rdf:resource="http://www.w3.org/2001/XMLSchema#string"/>
  </owl:DatatypeProperty>
  <owl:DatatypeProperty rdf:about="http://example.org/onto/prop/google_dialogflow_cx_webhook_parameter_mapping">
    <rdfs:label>parameter_mapping</rdfs:label>
    <rdfs:comment>Maps the values extracted from specific fields of the flexible webhook
response into session parameters.
- Key: session parameter name
- Value: field path in the webhook response</rdfs:comment>
    <rdfs:domain rdf:resource="http://example.org/onto/class/google_dialogflow_cx_webhook"/>
    <rdfs:range rdf:resource="http://www.w3.org/2001/XMLSchema#string"/>
  </owl:DatatypeProperty>
  <owl:DatatypeProperty rdf:about="http://example.org/onto/prop/google_dialogflow_cx_webhook_request_body">
    <rdfs:label>request_body</rdfs:label>
    <rdfs:comment>Defines a custom JSON object as request body to send to flexible webhook.</rdfs:comment>
    <rdfs:domain rdf:resource="http://example.org/onto/class/google_dialogflow_cx_webhook"/>
    <rdfs:range rdf:resource="http://www.w3.org/2001/XMLSchema#string"/>
  </owl:DatatypeProperty>
  <owl:DatatypeProperty rdf:about="http://example.org/onto/prop/google_dialogflow_cx_webhook_request_headers">
    <rdfs:label>request_headers</rdfs:label>
    <rdfs:comment>The HTTP request headers to send together with webhook requests.</rdfs:comment>
    <rdfs:domain rdf:resource="http://example.org/onto/class/google_dialogflow_cx_webhook"/>
    <rdfs:range rdf:resource="http://www.w3.org/2001/XMLSchema#string"/>
  </owl:DatatypeProperty>
  <owl:DatatypeProperty rdf:about="http://example.org/onto/prop/google_dialogflow_cx_webhook_secret_version_for_username_password">
    <rdfs:label>secret_version_for_username_password</rdfs:label>
    <rdfs:comment>The SecretManager secret version resource storing the username:password
pair for HTTP Basic authentication.
Format: 'projects/{project}/secrets/{secret}/versions/{version}'</rdfs:comment>
    <rdfs:domain rdf:resource="http://example.org/onto/class/google_dialogflow_cx_webhook"/>
    <rdfs:range rdf:resource="http://www.w3.org/2001/XMLSchema#string"/>
  </owl:DatatypeProperty>
  <owl:DatatypeProperty rdf:about="http://example.org/onto/prop/google_dialogflow_cx_webhook_service_agent_auth">
    <rdfs:label>service_agent_auth</rdfs:label>
    <rdfs:comment>Indicate the auth token type generated from the [Diglogflow service
agent](https://cloud.google.com/iam/docs/service-agents#dialogflow-service-agent).
The generated token is sent in the Authorization header. Possible values: ["NONE", "ID_TOKEN", "ACCESS_TOKEN"]</rdfs:comment>
    <rdfs:domain rdf:resource="http://example.org/onto/class/google_dialogflow_cx_webhook"/>
    <rdfs:range rdf:resource="http://www.w3.org/2001/XMLSchema#string"/>
  </owl:DatatypeProperty>
  <owl:DatatypeProperty rdf:about="http://example.org/onto/prop/google_dialogflow_cx_webhook_uri">
    <rdfs:label>uri</rdfs:label>
    <rdfs:comment>The webhook URI for receiving POST requests. It must use https protocol.</rdfs:comment>
    <rdfs:domain rdf:resource="http://example.org/onto/class/google_dialogflow_cx_webhook"/>
    <rdfs:range rdf:resource="http://www.w3.org/2001/XMLSchema#string"/>
  </owl:DatatypeProperty>
  <owl:DatatypeProperty rdf:about="http://example.org/onto/prop/google_dialogflow_cx_webhook_webhook_type">
    <rdfs:label>webhook_type</rdfs:label>
    <rdfs:comment>Type of the webhook. Possible values: ["STANDARD", "FLEXIBLE"]</rdfs:comment>
    <rdfs:domain rdf:resource="http://example.org/onto/class/google_dialogflow_cx_webhook"/>
    <rdfs:range rdf:resource="http://www.w3.org/2001/XMLSchema#string"/>
  </owl:DatatypeProperty>
  <owl:DatatypeProperty rdf:about="http://example.org/onto/prop/google_dialogflow_cx_webhook_client_id">
    <rdfs:label>client_id</rdfs:label>
    <rdfs:comment>The client ID provided by the 3rd party platform.</rdfs:comment>
    <rdfs:domain rdf:resource="http://example.org/onto/class/google_dialogflow_cx_webhook"/>
    <rdfs:range rdf:resource="http://www.w3.org/2001/XMLSchema#string"/>
  </owl:DatatypeProperty>
  <owl:DatatypeProperty rdf:about="http://example.org/onto/prop/google_dialogflow_cx_webhook_client_secret">
    <rdfs:label>client_secret</rdfs:label>
    <rdfs:comment>The client secret provided by the 3rd party platform.  If the
'secret_version_for_client_secret' field is set, this field will be
ignored.</rdfs:comment>
    <rdfs:domain rdf:resource="http://example.org/onto/class/google_dialogflow_cx_webhook"/>
    <rdfs:range rdf:resource="http://www.w3.org/2001/XMLSchema#string"/>
  </owl:DatatypeProperty>
  <owl:DatatypeProperty rdf:about="http://example.org/onto/prop/google_dialogflow_cx_webhook_scopes">
    <rdfs:label>scopes</rdfs:label>
    <rdfs:comment>The OAuth scopes to grant.</rdfs:comment>
    <rdfs:domain rdf:resource="http://example.org/onto/class/google_dialogflow_cx_webhook"/>
    <rdfs:range rdf:resource="http://www.w3.org/2001/XMLSchema#string"/>
  </owl:DatatypeProperty>
  <owl:DatatypeProperty rdf:about="http://example.org/onto/prop/google_dialogflow_cx_webhook_secret_version_for_client_secret">
    <rdfs:label>secret_version_for_client_secret</rdfs:label>
    <rdfs:comment>The name of the SecretManager secret version resource storing the
client secret. If this field is set, the 'client_secret' field will be
ignored.
Format: 'projects/{project}/secrets/{secret}/versions/{version}'</rdfs:comment>
    <rdfs:domain rdf:resource="http://example.org/onto/class/google_dialogflow_cx_webhook"/>
    <rdfs:range rdf:resource="http://www.w3.org/2001/XMLSchema#string"/>
  </owl:DatatypeProperty>
  <owl:DatatypeProperty rdf:about="http://example.org/onto/prop/google_dialogflow_cx_webhook_token_endpoint">
    <rdfs:label>token_endpoint</rdfs:label>
    <rdfs:comment>The token endpoint provided by the 3rd party platform to exchange an
access token.</rdfs:comment>
    <rdfs:domain rdf:resource="http://example.org/onto/class/google_dialogflow_cx_webhook"/>
    <rdfs:range rdf:resource="http://www.w3.org/2001/XMLSchema#string"/>
  </owl:DatatypeProperty>
  <owl:DatatypeProperty rdf:about="http://example.org/onto/prop/google_dialogflow_cx_webhook_key">
    <rdfs:label>key</rdfs:label>
    <rdfs:domain rdf:resource="http://example.org/onto/class/google_dialogflow_cx_webhook"/>
    <rdfs:range rdf:resource="http://www.w3.org/2001/XMLSchema#string"/>
  </owl:DatatypeProperty>
  <owl:DatatypeProperty rdf:about="http://example.org/onto/prop/google_dialogflow_cx_webhook_secret_version">
    <rdfs:label>secret_version</rdfs:label>
    <rdfs:comment>The SecretManager secret version resource storing the header value.
Format: 'projects/{project}/secrets/{secret}/versions/{version}'</rdfs:comment>
    <rdfs:domain rdf:resource="http://example.org/onto/class/google_dialogflow_cx_webhook"/>
    <rdfs:range rdf:resource="http://www.w3.org/2001/XMLSchema#string"/>
  </owl:DatatypeProperty>
  <owl:DatatypeProperty rdf:about="http://example.org/onto/prop/google_dialogflow_cx_webhook_create">
    <rdfs:label>create</rdfs:label>
    <rdfs:domain rdf:resource="http://example.org/onto/class/google_dialogflow_cx_webhook"/>
    <rdfs:range rdf:resource="http://www.w3.org/2001/XMLSchema#string"/>
  </owl:DatatypeProperty>
  <owl:DatatypeProperty rdf:about="http://example.org/onto/prop/google_dialogflow_cx_webhook_delete">
    <rdfs:label>delete</rdfs:label>
    <rdfs:domain rdf:resource="http://example.org/onto/class/google_dialogflow_cx_webhook"/>
    <rdfs:range rdf:resource="http://www.w3.org/2001/XMLSchema#string"/>
  </owl:DatatypeProperty>
  <owl:DatatypeProperty rdf:about="http://example.org/onto/prop/google_dialogflow_cx_webhook_update">
    <rdfs:label>update</rdfs:label>
    <rdfs:domain rdf:resource="http://example.org/onto/class/google_dialogflow_cx_webhook"/>
    <rdfs:range rdf:resource="http://www.w3.org/2001/XMLSchema#string"/>
  </owl:DatatypeProperty>
</rdf:RDF>
