<?xml version="1.0" encoding="UTF-8"?>
<rdf:RDF
  xmlns:rdf="http://www.w3.org/1999/02/22-rdf-syntax-ns#"
  xmlns:rdfs="http://www.w3.org/2000/01/rdf-schema#"
  xmlns:owl="http://www.w3.org/2002/07/owl#"
  xmlns:xsd="http://www.w3.org/2001/XMLSchema#"
  xml:base="http://example.org/onto/">
  <owl:Class rdf:about="http://example.org/onto/class/google_bigquery_data_transfer_config">
    <rdfs:label>google_bigquery_data_transfer_config</rdfs:label>
    <rdfs:comment>#
#     ***     AUTO GENERATED CODE    ***    Type: MMv1     ***
#
# ----------------------------------------------------------------------------
#
#     This code is generated by Magic Modules using the following:
#
#     Configuration: https:#github.com/GoogleCloudPlatform/magic-modules/tree/main/mmv1/products/bigquerydatatransfer/Config.yaml
#     Template:      https:#github.com/GoogleCloudPlatform/magic-modules/tree/main/mmv1/templates/terraform/resource.html.markdown.tmpl
#
#     DO NOT EDIT this file directly. Any changes made to this file will be
#     overwritten during the next generation cycle.
#
# ----------------------------------------------------------------------------
subcategory: "BigQuery Data Transfer"
description: |-
  Represents a data transfer configuration.
---</rdfs:comment>
  </owl:Class>
  <owl:DatatypeProperty rdf:about="http://example.org/onto/prop/google_bigquery_data_transfer_config_data_refresh_window_days">
    <rdfs:label>data_refresh_window_days</rdfs:label>
    <rdfs:comment>The number of days to look back to automatically refresh the data.
For example, if dataRefreshWindowDays = 10, then every day BigQuery
reingests data for [today-10, today-1], rather than ingesting data for
just [today-1]. Only valid if the data source supports the feature.
Set the value to 0 to use the default value.</rdfs:comment>
    <rdfs:domain rdf:resource="http://example.org/onto/class/google_bigquery_data_transfer_config"/>
    <rdfs:range rdf:resource="http://www.w3.org/2001/XMLSchema#string"/>
  </owl:DatatypeProperty>
  <owl:DatatypeProperty rdf:about="http://example.org/onto/prop/google_bigquery_data_transfer_config_data_source_id">
    <rdfs:label>data_source_id</rdfs:label>
    <rdfs:comment>The data source id. Cannot be changed once the transfer config is created.</rdfs:comment>
    <rdfs:domain rdf:resource="http://example.org/onto/class/google_bigquery_data_transfer_config"/>
    <rdfs:range rdf:resource="http://www.w3.org/2001/XMLSchema#string"/>
  </owl:DatatypeProperty>
  <owl:DatatypeProperty rdf:about="http://example.org/onto/prop/google_bigquery_data_transfer_config_destination_dataset_id">
    <rdfs:label>destination_dataset_id</rdfs:label>
    <rdfs:comment>The BigQuery target dataset id.</rdfs:comment>
    <rdfs:domain rdf:resource="http://example.org/onto/class/google_bigquery_data_transfer_config"/>
    <rdfs:range rdf:resource="http://www.w3.org/2001/XMLSchema#string"/>
  </owl:DatatypeProperty>
  <owl:DatatypeProperty rdf:about="http://example.org/onto/prop/google_bigquery_data_transfer_config_disabled">
    <rdfs:label>disabled</rdfs:label>
    <rdfs:comment>When set to true, no runs are scheduled for a given transfer.</rdfs:comment>
    <rdfs:domain rdf:resource="http://example.org/onto/class/google_bigquery_data_transfer_config"/>
    <rdfs:range rdf:resource="http://www.w3.org/2001/XMLSchema#string"/>
  </owl:DatatypeProperty>
  <owl:DatatypeProperty rdf:about="http://example.org/onto/prop/google_bigquery_data_transfer_config_display_name">
    <rdfs:label>display_name</rdfs:label>
    <rdfs:comment>The user specified display name for the transfer config.</rdfs:comment>
    <rdfs:domain rdf:resource="http://example.org/onto/class/google_bigquery_data_transfer_config"/>
    <rdfs:range rdf:resource="http://www.w3.org/2001/XMLSchema#string"/>
  </owl:DatatypeProperty>
  <owl:DatatypeProperty rdf:about="http://example.org/onto/prop/google_bigquery_data_transfer_config_id">
    <rdfs:label>id</rdfs:label>
    <rdfs:domain rdf:resource="http://example.org/onto/class/google_bigquery_data_transfer_config"/>
    <rdfs:range rdf:resource="http://www.w3.org/2001/XMLSchema#string"/>
  </owl:DatatypeProperty>
  <owl:DatatypeProperty rdf:about="http://example.org/onto/prop/google_bigquery_data_transfer_config_location">
    <rdfs:label>location</rdfs:label>
    <rdfs:comment>The geographic location where the transfer config should reside.
Examples: US, EU, asia-northeast1. The default value is US.</rdfs:comment>
    <rdfs:domain rdf:resource="http://example.org/onto/class/google_bigquery_data_transfer_config"/>
    <rdfs:range rdf:resource="http://www.w3.org/2001/XMLSchema#string"/>
  </owl:DatatypeProperty>
  <owl:DatatypeProperty rdf:about="http://example.org/onto/prop/google_bigquery_data_transfer_config_name">
    <rdfs:label>name</rdfs:label>
    <rdfs:comment>The resource name of the transfer config. Transfer config names have the
form projects/{projectId}/locations/{location}/transferConfigs/{configId}
or projects/{projectId}/transferConfigs/{configId},
where configId is usually a uuid, but this is not required.
The name is ignored when creating a transfer config.</rdfs:comment>
    <rdfs:domain rdf:resource="http://example.org/onto/class/google_bigquery_data_transfer_config"/>
    <rdfs:range rdf:resource="http://www.w3.org/2001/XMLSchema#string"/>
  </owl:DatatypeProperty>
  <owl:DatatypeProperty rdf:about="http://example.org/onto/prop/google_bigquery_data_transfer_config_notification_pubsub_topic">
    <rdfs:label>notification_pubsub_topic</rdfs:label>
    <rdfs:comment>Pub/Sub topic where notifications will be sent after transfer runs
associated with this transfer config finish.</rdfs:comment>
    <rdfs:domain rdf:resource="http://example.org/onto/class/google_bigquery_data_transfer_config"/>
    <rdfs:range rdf:resource="http://www.w3.org/2001/XMLSchema#string"/>
  </owl:DatatypeProperty>
  <owl:DatatypeProperty rdf:about="http://example.org/onto/prop/google_bigquery_data_transfer_config_params">
    <rdfs:label>params</rdfs:label>
    <rdfs:comment>Parameters specific to each data source. For more information see the bq tab in the 'Setting up a data transfer'
section for each data source. For example the parameters for Cloud Storage transfers are listed here:
https://cloud.google.com/bigquery-transfer/docs/cloud-storage-transfer#bq

**NOTE** : If you are attempting to update a parameter that cannot be updated (due to api limitations) [please force recreation of the resource](https://www.terraform.io/cli/state/taint#forcing-re-creation-of-resources).</rdfs:comment>
    <rdfs:domain rdf:resource="http://example.org/onto/class/google_bigquery_data_transfer_config"/>
    <rdfs:range rdf:resource="http://www.w3.org/2001/XMLSchema#string"/>
  </owl:DatatypeProperty>
  <owl:DatatypeProperty rdf:about="http://example.org/onto/prop/google_bigquery_data_transfer_config_project">
    <rdfs:label>project</rdfs:label>
    <rdfs:domain rdf:resource="http://example.org/onto/class/google_bigquery_data_transfer_config"/>
    <rdfs:range rdf:resource="http://www.w3.org/2001/XMLSchema#string"/>
  </owl:DatatypeProperty>
  <owl:DatatypeProperty rdf:about="http://example.org/onto/prop/google_bigquery_data_transfer_config_schedule">
    <rdfs:label>schedule</rdfs:label>
    <rdfs:comment>Data transfer schedule. If the data source does not support a custom
schedule, this should be empty. If it is empty, the default value for
the data source will be used. The specified times are in UTC. Examples
of valid format: 1st,3rd monday of month 15:30, every wed,fri of jan,
jun 13:15, and first sunday of quarter 00:00. See more explanation
about the format here:
https://cloud.google.com/appengine/docs/flexible/python/scheduling-jobs-with-cron-yaml#the_schedule_format
NOTE: The minimum interval time between recurring transfers depends
on the data source; refer to the documentation for your data source.</rdfs:comment>
    <rdfs:domain rdf:resource="http://example.org/onto/class/google_bigquery_data_transfer_config"/>
    <rdfs:range rdf:resource="http://www.w3.org/2001/XMLSchema#string"/>
  </owl:DatatypeProperty>
  <owl:DatatypeProperty rdf:about="http://example.org/onto/prop/google_bigquery_data_transfer_config_service_account_name">
    <rdfs:label>service_account_name</rdfs:label>
    <rdfs:comment>Service account email. If this field is set, transfer config will
be created with this service account credentials. It requires that
requesting user calling this API has permissions to act as this service account.</rdfs:comment>
    <rdfs:domain rdf:resource="http://example.org/onto/class/google_bigquery_data_transfer_config"/>
    <rdfs:range rdf:resource="http://www.w3.org/2001/XMLSchema#string"/>
  </owl:DatatypeProperty>
  <owl:DatatypeProperty rdf:about="http://example.org/onto/prop/google_bigquery_data_transfer_config_enable_failure_email">
    <rdfs:label>enable_failure_email</rdfs:label>
    <rdfs:comment>If true, email notifications will be sent on transfer run failures.</rdfs:comment>
    <rdfs:domain rdf:resource="http://example.org/onto/class/google_bigquery_data_transfer_config"/>
    <rdfs:range rdf:resource="http://www.w3.org/2001/XMLSchema#string"/>
  </owl:DatatypeProperty>
  <owl:DatatypeProperty rdf:about="http://example.org/onto/prop/google_bigquery_data_transfer_config_kms_key_name">
    <rdfs:label>kms_key_name</rdfs:label>
    <rdfs:comment>The name of the KMS key used for encrypting BigQuery data.</rdfs:comment>
    <rdfs:domain rdf:resource="http://example.org/onto/class/google_bigquery_data_transfer_config"/>
    <rdfs:range rdf:resource="http://www.w3.org/2001/XMLSchema#string"/>
  </owl:DatatypeProperty>
  <owl:DatatypeProperty rdf:about="http://example.org/onto/prop/google_bigquery_data_transfer_config_disable_auto_scheduling">
    <rdfs:label>disable_auto_scheduling</rdfs:label>
    <rdfs:comment>If true, automatic scheduling of data transfer runs for this
configuration will be disabled. The runs can be started on ad-hoc
basis using transferConfigs.startManualRuns API. When automatic
scheduling is disabled, the TransferConfig.schedule field will
be ignored.</rdfs:comment>
    <rdfs:domain rdf:resource="http://example.org/onto/class/google_bigquery_data_transfer_config"/>
    <rdfs:range rdf:resource="http://www.w3.org/2001/XMLSchema#string"/>
  </owl:DatatypeProperty>
  <owl:DatatypeProperty rdf:about="http://example.org/onto/prop/google_bigquery_data_transfer_config_end_time">
    <rdfs:label>end_time</rdfs:label>
    <rdfs:comment>Defines time to stop scheduling transfer runs. A transfer run cannot be
scheduled at or after the end time. The end time can be changed at any
moment. The time when a data transfer can be triggered manually is not
limited by this option.</rdfs:comment>
    <rdfs:domain rdf:resource="http://example.org/onto/class/google_bigquery_data_transfer_config"/>
    <rdfs:range rdf:resource="http://www.w3.org/2001/XMLSchema#string"/>
  </owl:DatatypeProperty>
  <owl:DatatypeProperty rdf:about="http://example.org/onto/prop/google_bigquery_data_transfer_config_start_time">
    <rdfs:label>start_time</rdfs:label>
    <rdfs:comment>Specifies time to start scheduling transfer runs. The first run will be
scheduled at or after the start time according to a recurrence pattern
defined in the schedule string. The start time can be changed at any
moment. The time when a data transfer can be triggered manually is not
limited by this option.</rdfs:comment>
    <rdfs:domain rdf:resource="http://example.org/onto/class/google_bigquery_data_transfer_config"/>
    <rdfs:range rdf:resource="http://www.w3.org/2001/XMLSchema#string"/>
  </owl:DatatypeProperty>
  <owl:DatatypeProperty rdf:about="http://example.org/onto/prop/google_bigquery_data_transfer_config_secret_access_key">
    <rdfs:label>secret_access_key</rdfs:label>
    <rdfs:comment>The Secret Access Key of the AWS account transferring data from.</rdfs:comment>
    <rdfs:domain rdf:resource="http://example.org/onto/class/google_bigquery_data_transfer_config"/>
    <rdfs:range rdf:resource="http://www.w3.org/2001/XMLSchema#string"/>
  </owl:DatatypeProperty>
  <owl:DatatypeProperty rdf:about="http://example.org/onto/prop/google_bigquery_data_transfer_config_secret_access_key_wo">
    <rdfs:label>secret_access_key_wo</rdfs:label>
    <rdfs:comment>The Secret Access Key of the AWS account transferring data from.</rdfs:comment>
    <rdfs:domain rdf:resource="http://example.org/onto/class/google_bigquery_data_transfer_config"/>
    <rdfs:range rdf:resource="http://www.w3.org/2001/XMLSchema#string"/>
  </owl:DatatypeProperty>
  <owl:DatatypeProperty rdf:about="http://example.org/onto/prop/google_bigquery_data_transfer_config_secret_access_key_wo_version">
    <rdfs:label>secret_access_key_wo_version</rdfs:label>
    <rdfs:comment>The version of the sensitive params - used to trigger updates of the write-only params. For more info see [updating write-only attributes](/docs/providers/google/guides/using_write_only_attributes.html#updating-write-only-attributes)</rdfs:comment>
    <rdfs:domain rdf:resource="http://example.org/onto/class/google_bigquery_data_transfer_config"/>
    <rdfs:range rdf:resource="http://www.w3.org/2001/XMLSchema#string"/>
  </owl:DatatypeProperty>
  <owl:DatatypeProperty rdf:about="http://example.org/onto/prop/google_bigquery_data_transfer_config_create">
    <rdfs:label>create</rdfs:label>
    <rdfs:domain rdf:resource="http://example.org/onto/class/google_bigquery_data_transfer_config"/>
    <rdfs:range rdf:resource="http://www.w3.org/2001/XMLSchema#string"/>
  </owl:DatatypeProperty>
  <owl:DatatypeProperty rdf:about="http://example.org/onto/prop/google_bigquery_data_transfer_config_delete">
    <rdfs:label>delete</rdfs:label>
    <rdfs:domain rdf:resource="http://example.org/onto/class/google_bigquery_data_transfer_config"/>
    <rdfs:range rdf:resource="http://www.w3.org/2001/XMLSchema#string"/>
  </owl:DatatypeProperty>
  <owl:DatatypeProperty rdf:about="http://example.org/onto/prop/google_bigquery_data_transfer_config_update">
    <rdfs:label>update</rdfs:label>
    <rdfs:domain rdf:resource="http://example.org/onto/class/google_bigquery_data_transfer_config"/>
    <rdfs:range rdf:resource="http://www.w3.org/2001/XMLSchema#string"/>
  </owl:DatatypeProperty>
</rdf:RDF>
