<?xml version="1.0" encoding="UTF-8"?>
<rdf:RDF
  xmlns:rdf="http://www.w3.org/1999/02/22-rdf-syntax-ns#"
  xmlns:rdfs="http://www.w3.org/2000/01/rdf-schema#"
  xmlns:owl="http://www.w3.org/2002/07/owl#"
  xmlns:xsd="http://www.w3.org/2001/XMLSchema#"
  xml:base="http://example.org/onto/">
  <owl:Class rdf:about="http://example.org/onto/class/google_dialogflow_cx_playbook">
    <rdfs:label>google_dialogflow_cx_playbook</rdfs:label>
    <rdfs:comment>#
#     ***     AUTO GENERATED CODE    ***    Type: MMv1     ***
#
# ----------------------------------------------------------------------------
#
#     This code is generated by Magic Modules using the following:
#
#     Configuration: https:#github.com/GoogleCloudPlatform/magic-modules/tree/main/mmv1/products/dialogflowcx/Playbook.yaml
#     Template:      https:#github.com/GoogleCloudPlatform/magic-modules/tree/main/mmv1/templates/terraform/resource.html.markdown.tmpl
#
#     DO NOT EDIT this file directly. Any changes made to this file will be
#     overwritten during the next generation cycle.
#
# ----------------------------------------------------------------------------
subcategory: "Dialogflow CX"
description: |-
  Playbook is the basic building block to instruct the LLM how to execute a certain task.
---</rdfs:comment>
  </owl:Class>
  <owl:DatatypeProperty rdf:about="http://example.org/onto/prop/google_dialogflow_cx_playbook_create_time">
    <rdfs:label>create_time</rdfs:label>
    <rdfs:comment>The timestamp of initial playbook creation.

Uses RFC 3339, where generated output will always be Z-normalized and uses 0, 3, 6 or 9 fractional digits. Offsets other than "Z" are also accepted. Examples: "2014-10-02T15:01:23Z", "2014-10-02T15:01:23.045123456Z" or "2014-10-02T15:01:23+05:30".</rdfs:comment>
    <rdfs:domain rdf:resource="http://example.org/onto/class/google_dialogflow_cx_playbook"/>
    <rdfs:range rdf:resource="http://www.w3.org/2001/XMLSchema#string"/>
  </owl:DatatypeProperty>
  <owl:DatatypeProperty rdf:about="http://example.org/onto/prop/google_dialogflow_cx_playbook_display_name">
    <rdfs:label>display_name</rdfs:label>
    <rdfs:comment>The human-readable name of the playbook, unique within an agent.</rdfs:comment>
    <rdfs:domain rdf:resource="http://example.org/onto/class/google_dialogflow_cx_playbook"/>
    <rdfs:range rdf:resource="http://www.w3.org/2001/XMLSchema#string"/>
  </owl:DatatypeProperty>
  <owl:DatatypeProperty rdf:about="http://example.org/onto/prop/google_dialogflow_cx_playbook_goal">
    <rdfs:label>goal</rdfs:label>
    <rdfs:comment>High level description of the goal the playbook intend to accomplish. A goal should be concise since it's visible to other playbooks that may reference this playbook.</rdfs:comment>
    <rdfs:domain rdf:resource="http://example.org/onto/class/google_dialogflow_cx_playbook"/>
    <rdfs:range rdf:resource="http://www.w3.org/2001/XMLSchema#string"/>
  </owl:DatatypeProperty>
  <owl:DatatypeProperty rdf:about="http://example.org/onto/prop/google_dialogflow_cx_playbook_id">
    <rdfs:label>id</rdfs:label>
    <rdfs:domain rdf:resource="http://example.org/onto/class/google_dialogflow_cx_playbook"/>
    <rdfs:range rdf:resource="http://www.w3.org/2001/XMLSchema#string"/>
  </owl:DatatypeProperty>
  <owl:DatatypeProperty rdf:about="http://example.org/onto/prop/google_dialogflow_cx_playbook_name">
    <rdfs:label>name</rdfs:label>
    <rdfs:comment>The unique identifier of the Playbook.
Format: projects/<Project ID>/locations/<Location ID>/agents/<Agent ID>/playbooks/<Playbook ID>.</rdfs:comment>
    <rdfs:domain rdf:resource="http://example.org/onto/class/google_dialogflow_cx_playbook"/>
    <rdfs:range rdf:resource="http://www.w3.org/2001/XMLSchema#string"/>
  </owl:DatatypeProperty>
  <owl:DatatypeProperty rdf:about="http://example.org/onto/prop/google_dialogflow_cx_playbook_parent">
    <rdfs:label>parent</rdfs:label>
    <rdfs:comment>The agent to create a Playbook for.
Format: projects/<Project ID>/locations/<Location ID>/agents/<Agent ID>.</rdfs:comment>
    <rdfs:domain rdf:resource="http://example.org/onto/class/google_dialogflow_cx_playbook"/>
    <rdfs:range rdf:resource="http://www.w3.org/2001/XMLSchema#string"/>
  </owl:DatatypeProperty>
  <owl:DatatypeProperty rdf:about="http://example.org/onto/prop/google_dialogflow_cx_playbook_playbook_type">
    <rdfs:label>playbook_type</rdfs:label>
    <rdfs:comment>Type of the playbook. Possible values: ["PLAYBOOK_TYPE_UNSPECIFIED", "TASK", "ROUTINE"]</rdfs:comment>
    <rdfs:domain rdf:resource="http://example.org/onto/class/google_dialogflow_cx_playbook"/>
    <rdfs:range rdf:resource="http://www.w3.org/2001/XMLSchema#string"/>
  </owl:DatatypeProperty>
  <owl:DatatypeProperty rdf:about="http://example.org/onto/prop/google_dialogflow_cx_playbook_referenced_flows">
    <rdfs:label>referenced_flows</rdfs:label>
    <rdfs:comment>The resource name of flows referenced by the current playbook in the instructions.</rdfs:comment>
    <rdfs:domain rdf:resource="http://example.org/onto/class/google_dialogflow_cx_playbook"/>
    <rdfs:range rdf:resource="http://www.w3.org/2001/XMLSchema#string"/>
  </owl:DatatypeProperty>
  <owl:DatatypeProperty rdf:about="http://example.org/onto/prop/google_dialogflow_cx_playbook_referenced_playbooks">
    <rdfs:label>referenced_playbooks</rdfs:label>
    <rdfs:comment>The resource name of other playbooks referenced by the current playbook in the instructions.</rdfs:comment>
    <rdfs:domain rdf:resource="http://example.org/onto/class/google_dialogflow_cx_playbook"/>
    <rdfs:range rdf:resource="http://www.w3.org/2001/XMLSchema#string"/>
  </owl:DatatypeProperty>
  <owl:DatatypeProperty rdf:about="http://example.org/onto/prop/google_dialogflow_cx_playbook_referenced_tools">
    <rdfs:label>referenced_tools</rdfs:label>
    <rdfs:comment>The resource name of tools referenced by the current playbook in the instructions. If not provided explicitly, they are will be implied using the tool being referenced in goal and steps.</rdfs:comment>
    <rdfs:domain rdf:resource="http://example.org/onto/class/google_dialogflow_cx_playbook"/>
    <rdfs:range rdf:resource="http://www.w3.org/2001/XMLSchema#string"/>
  </owl:DatatypeProperty>
  <owl:DatatypeProperty rdf:about="http://example.org/onto/prop/google_dialogflow_cx_playbook_token_count">
    <rdfs:label>token_count</rdfs:label>
    <rdfs:comment>Estimated number of tokes current playbook takes when sent to the LLM.</rdfs:comment>
    <rdfs:domain rdf:resource="http://example.org/onto/class/google_dialogflow_cx_playbook"/>
    <rdfs:range rdf:resource="http://www.w3.org/2001/XMLSchema#string"/>
  </owl:DatatypeProperty>
  <owl:DatatypeProperty rdf:about="http://example.org/onto/prop/google_dialogflow_cx_playbook_update_time">
    <rdfs:label>update_time</rdfs:label>
    <rdfs:comment>Last time the playbook version was updated.

Uses RFC 3339, where generated output will always be Z-normalized and uses 0, 3, 6 or 9 fractional digits. Offsets other than "Z" are also accepted. Examples: "2014-10-02T15:01:23Z", "2014-10-02T15:01:23.045123456Z" or "2014-10-02T15:01:23+05:30".</rdfs:comment>
    <rdfs:domain rdf:resource="http://example.org/onto/class/google_dialogflow_cx_playbook"/>
    <rdfs:range rdf:resource="http://www.w3.org/2001/XMLSchema#string"/>
  </owl:DatatypeProperty>
  <owl:DatatypeProperty rdf:about="http://example.org/onto/prop/google_dialogflow_cx_playbook_guidelines">
    <rdfs:label>guidelines</rdfs:label>
    <rdfs:comment>General guidelines for the playbook. These are unstructured instructions that are not directly part of the goal, e.g. "Always be polite". It's valid for this text to be long and used instead of steps altogether.</rdfs:comment>
    <rdfs:domain rdf:resource="http://example.org/onto/class/google_dialogflow_cx_playbook"/>
    <rdfs:range rdf:resource="http://www.w3.org/2001/XMLSchema#string"/>
  </owl:DatatypeProperty>
  <owl:DatatypeProperty rdf:about="http://example.org/onto/prop/google_dialogflow_cx_playbook_steps">
    <rdfs:label>steps</rdfs:label>
    <rdfs:comment>Sub-processing needed to execute the current step.

This field uses JSON data as a string. The value provided must be a valid JSON representation documented in [Step](https://cloud.google.com/dialogflow/cx/docs/reference/rest/v3/projects.locations.agents.playbooks#step).</rdfs:comment>
    <rdfs:domain rdf:resource="http://example.org/onto/class/google_dialogflow_cx_playbook"/>
    <rdfs:range rdf:resource="http://www.w3.org/2001/XMLSchema#string"/>
  </owl:DatatypeProperty>
  <owl:DatatypeProperty rdf:about="http://example.org/onto/prop/google_dialogflow_cx_playbook_text">
    <rdfs:label>text</rdfs:label>
    <rdfs:comment>Step instruction in text format.</rdfs:comment>
    <rdfs:domain rdf:resource="http://example.org/onto/class/google_dialogflow_cx_playbook"/>
    <rdfs:range rdf:resource="http://www.w3.org/2001/XMLSchema#string"/>
  </owl:DatatypeProperty>
  <owl:DatatypeProperty rdf:about="http://example.org/onto/prop/google_dialogflow_cx_playbook_model">
    <rdfs:label>model</rdfs:label>
    <rdfs:comment>The selected LLM model.</rdfs:comment>
    <rdfs:domain rdf:resource="http://example.org/onto/class/google_dialogflow_cx_playbook"/>
    <rdfs:range rdf:resource="http://www.w3.org/2001/XMLSchema#string"/>
  </owl:DatatypeProperty>
  <owl:DatatypeProperty rdf:about="http://example.org/onto/prop/google_dialogflow_cx_playbook_prompt_text">
    <rdfs:label>prompt_text</rdfs:label>
    <rdfs:comment>The custom prompt to use.</rdfs:comment>
    <rdfs:domain rdf:resource="http://example.org/onto/class/google_dialogflow_cx_playbook"/>
    <rdfs:range rdf:resource="http://www.w3.org/2001/XMLSchema#string"/>
  </owl:DatatypeProperty>
  <owl:DatatypeProperty rdf:about="http://example.org/onto/prop/google_dialogflow_cx_playbook_create">
    <rdfs:label>create</rdfs:label>
    <rdfs:domain rdf:resource="http://example.org/onto/class/google_dialogflow_cx_playbook"/>
    <rdfs:range rdf:resource="http://www.w3.org/2001/XMLSchema#string"/>
  </owl:DatatypeProperty>
  <owl:DatatypeProperty rdf:about="http://example.org/onto/prop/google_dialogflow_cx_playbook_delete">
    <rdfs:label>delete</rdfs:label>
    <rdfs:domain rdf:resource="http://example.org/onto/class/google_dialogflow_cx_playbook"/>
    <rdfs:range rdf:resource="http://www.w3.org/2001/XMLSchema#string"/>
  </owl:DatatypeProperty>
  <owl:DatatypeProperty rdf:about="http://example.org/onto/prop/google_dialogflow_cx_playbook_update">
    <rdfs:label>update</rdfs:label>
    <rdfs:domain rdf:resource="http://example.org/onto/class/google_dialogflow_cx_playbook"/>
    <rdfs:range rdf:resource="http://www.w3.org/2001/XMLSchema#string"/>
  </owl:DatatypeProperty>
</rdf:RDF>
