<?xml version="1.0" encoding="UTF-8"?>
<rdf:RDF
  xmlns:rdf="http://www.w3.org/1999/02/22-rdf-syntax-ns#"
  xmlns:rdfs="http://www.w3.org/2000/01/rdf-schema#"
  xmlns:owl="http://www.w3.org/2002/07/owl#"
  xmlns:xsd="http://www.w3.org/2001/XMLSchema#"
  xml:base="http://example.org/onto/">
  <owl:Class rdf:about="http://example.org/onto/class/google_compute_backend_bucket">
    <rdfs:label>google_compute_backend_bucket</rdfs:label>
    <rdfs:comment>#
#     ***     AUTO GENERATED CODE    ***    Type: MMv1     ***
#
# ----------------------------------------------------------------------------
#
#     This code is generated by Magic Modules using the following:
#
#     Configuration: https:#github.com/GoogleCloudPlatform/magic-modules/tree/main/mmv1/products/compute/BackendBucket.yaml
#     Template:      https:#github.com/GoogleCloudPlatform/magic-modules/tree/main/mmv1/templates/terraform/resource.html.markdown.tmpl
#
#     DO NOT EDIT this file directly. Any changes made to this file will be
#     overwritten during the next generation cycle.
#
# ----------------------------------------------------------------------------
subcategory: "Compute Engine"
description: |-
  Backend buckets allow you to use Google Cloud Storage buckets with HTTP(S)
  load balancing.
---</rdfs:comment>
  </owl:Class>
  <owl:DatatypeProperty rdf:about="http://example.org/onto/prop/google_compute_backend_bucket_bucket_name">
    <rdfs:label>bucket_name</rdfs:label>
    <rdfs:comment>Cloud Storage bucket name.</rdfs:comment>
    <rdfs:domain rdf:resource="http://example.org/onto/class/google_compute_backend_bucket"/>
    <rdfs:range rdf:resource="http://www.w3.org/2001/XMLSchema#string"/>
  </owl:DatatypeProperty>
  <owl:DatatypeProperty rdf:about="http://example.org/onto/prop/google_compute_backend_bucket_compression_mode">
    <rdfs:label>compression_mode</rdfs:label>
    <rdfs:comment>Compress text responses using Brotli or gzip compression, based on the client's Accept-Encoding header. Possible values: ["AUTOMATIC", "DISABLED"]</rdfs:comment>
    <rdfs:domain rdf:resource="http://example.org/onto/class/google_compute_backend_bucket"/>
    <rdfs:range rdf:resource="http://www.w3.org/2001/XMLSchema#string"/>
  </owl:DatatypeProperty>
  <owl:DatatypeProperty rdf:about="http://example.org/onto/prop/google_compute_backend_bucket_creation_timestamp">
    <rdfs:label>creation_timestamp</rdfs:label>
    <rdfs:comment>Creation timestamp in RFC3339 text format.</rdfs:comment>
    <rdfs:domain rdf:resource="http://example.org/onto/class/google_compute_backend_bucket"/>
    <rdfs:range rdf:resource="http://www.w3.org/2001/XMLSchema#string"/>
  </owl:DatatypeProperty>
  <owl:DatatypeProperty rdf:about="http://example.org/onto/prop/google_compute_backend_bucket_custom_response_headers">
    <rdfs:label>custom_response_headers</rdfs:label>
    <rdfs:comment>Headers that the HTTP/S load balancer should add to proxied responses.</rdfs:comment>
    <rdfs:domain rdf:resource="http://example.org/onto/class/google_compute_backend_bucket"/>
    <rdfs:range rdf:resource="http://www.w3.org/2001/XMLSchema#string"/>
  </owl:DatatypeProperty>
  <owl:DatatypeProperty rdf:about="http://example.org/onto/prop/google_compute_backend_bucket_description">
    <rdfs:label>description</rdfs:label>
    <rdfs:comment>An optional textual description of the resource; provided by the
client when the resource is created.</rdfs:comment>
    <rdfs:domain rdf:resource="http://example.org/onto/class/google_compute_backend_bucket"/>
    <rdfs:range rdf:resource="http://www.w3.org/2001/XMLSchema#string"/>
  </owl:DatatypeProperty>
  <owl:DatatypeProperty rdf:about="http://example.org/onto/prop/google_compute_backend_bucket_edge_security_policy">
    <rdfs:label>edge_security_policy</rdfs:label>
    <rdfs:comment>The security policy associated with this backend bucket.</rdfs:comment>
    <rdfs:domain rdf:resource="http://example.org/onto/class/google_compute_backend_bucket"/>
    <rdfs:range rdf:resource="http://www.w3.org/2001/XMLSchema#string"/>
  </owl:DatatypeProperty>
  <owl:DatatypeProperty rdf:about="http://example.org/onto/prop/google_compute_backend_bucket_enable_cdn">
    <rdfs:label>enable_cdn</rdfs:label>
    <rdfs:comment>If true, enable Cloud CDN for this BackendBucket.
Note: This cannot be set to true when loadBalancingScheme is set to INTERNAL_MANAGED.</rdfs:comment>
    <rdfs:domain rdf:resource="http://example.org/onto/class/google_compute_backend_bucket"/>
    <rdfs:range rdf:resource="http://www.w3.org/2001/XMLSchema#string"/>
  </owl:DatatypeProperty>
  <owl:DatatypeProperty rdf:about="http://example.org/onto/prop/google_compute_backend_bucket_id">
    <rdfs:label>id</rdfs:label>
    <rdfs:domain rdf:resource="http://example.org/onto/class/google_compute_backend_bucket"/>
    <rdfs:range rdf:resource="http://www.w3.org/2001/XMLSchema#string"/>
  </owl:DatatypeProperty>
  <owl:DatatypeProperty rdf:about="http://example.org/onto/prop/google_compute_backend_bucket_load_balancing_scheme">
    <rdfs:label>load_balancing_scheme</rdfs:label>
    <rdfs:comment>The value can only be INTERNAL_MANAGED for cross-region internal layer 7 load balancer.
If loadBalancingScheme is not specified, the backend bucket can be used by classic global external load balancers, or global application external load balancers, or both.
Important: CDN cannot be enabled (enableCdn cannot be set to true) when loadBalancingScheme is set to INTERNAL_MANAGED. Possible values: ["INTERNAL_MANAGED"]</rdfs:comment>
    <rdfs:domain rdf:resource="http://example.org/onto/class/google_compute_backend_bucket"/>
    <rdfs:range rdf:resource="http://www.w3.org/2001/XMLSchema#string"/>
  </owl:DatatypeProperty>
  <owl:DatatypeProperty rdf:about="http://example.org/onto/prop/google_compute_backend_bucket_name">
    <rdfs:label>name</rdfs:label>
    <rdfs:comment>Name of the resource. Provided by the client when the resource is
created. The name must be 1-63 characters long, and comply with
RFC1035.  Specifically, the name must be 1-63 characters long and
match the regular expression '[a-z]([-a-z0-9]*[a-z0-9])?' which means
the first character must be a lowercase letter, and all following
characters must be a dash, lowercase letter, or digit, except the
last character, which cannot be a dash.</rdfs:comment>
    <rdfs:domain rdf:resource="http://example.org/onto/class/google_compute_backend_bucket"/>
    <rdfs:range rdf:resource="http://www.w3.org/2001/XMLSchema#string"/>
  </owl:DatatypeProperty>
  <owl:DatatypeProperty rdf:about="http://example.org/onto/prop/google_compute_backend_bucket_project">
    <rdfs:label>project</rdfs:label>
    <rdfs:domain rdf:resource="http://example.org/onto/class/google_compute_backend_bucket"/>
    <rdfs:range rdf:resource="http://www.w3.org/2001/XMLSchema#string"/>
  </owl:DatatypeProperty>
  <owl:DatatypeProperty rdf:about="http://example.org/onto/prop/google_compute_backend_bucket_self_link">
    <rdfs:label>self_link</rdfs:label>
    <rdfs:domain rdf:resource="http://example.org/onto/class/google_compute_backend_bucket"/>
    <rdfs:range rdf:resource="http://www.w3.org/2001/XMLSchema#string"/>
  </owl:DatatypeProperty>
  <owl:DatatypeProperty rdf:about="http://example.org/onto/prop/google_compute_backend_bucket_cache_mode">
    <rdfs:label>cache_mode</rdfs:label>
    <rdfs:comment>Specifies the cache setting for all responses from this backend.
The possible values are: USE_ORIGIN_HEADERS, FORCE_CACHE_ALL and CACHE_ALL_STATIC Possible values: ["USE_ORIGIN_HEADERS", "FORCE_CACHE_ALL", "CACHE_ALL_STATIC"]</rdfs:comment>
    <rdfs:domain rdf:resource="http://example.org/onto/class/google_compute_backend_bucket"/>
    <rdfs:range rdf:resource="http://www.w3.org/2001/XMLSchema#string"/>
  </owl:DatatypeProperty>
  <owl:DatatypeProperty rdf:about="http://example.org/onto/prop/google_compute_backend_bucket_client_ttl">
    <rdfs:label>client_ttl</rdfs:label>
    <rdfs:comment>Specifies the maximum allowed TTL for cached content served by this origin. When the
'cache_mode' is set to "USE_ORIGIN_HEADERS", you must omit this field.</rdfs:comment>
    <rdfs:domain rdf:resource="http://example.org/onto/class/google_compute_backend_bucket"/>
    <rdfs:range rdf:resource="http://www.w3.org/2001/XMLSchema#string"/>
  </owl:DatatypeProperty>
  <owl:DatatypeProperty rdf:about="http://example.org/onto/prop/google_compute_backend_bucket_default_ttl">
    <rdfs:label>default_ttl</rdfs:label>
    <rdfs:comment>Specifies the default TTL for cached content served by this origin for responses
that do not have an existing valid TTL (max-age or s-max-age). When the 'cache_mode'
is set to "USE_ORIGIN_HEADERS", you must omit this field.</rdfs:comment>
    <rdfs:domain rdf:resource="http://example.org/onto/class/google_compute_backend_bucket"/>
    <rdfs:range rdf:resource="http://www.w3.org/2001/XMLSchema#string"/>
  </owl:DatatypeProperty>
  <owl:DatatypeProperty rdf:about="http://example.org/onto/prop/google_compute_backend_bucket_max_ttl">
    <rdfs:label>max_ttl</rdfs:label>
    <rdfs:comment>Specifies the maximum allowed TTL for cached content served by this origin. When the
'cache_mode' is set to "USE_ORIGIN_HEADERS", you must omit this field.</rdfs:comment>
    <rdfs:domain rdf:resource="http://example.org/onto/class/google_compute_backend_bucket"/>
    <rdfs:range rdf:resource="http://www.w3.org/2001/XMLSchema#string"/>
  </owl:DatatypeProperty>
  <owl:DatatypeProperty rdf:about="http://example.org/onto/prop/google_compute_backend_bucket_negative_caching">
    <rdfs:label>negative_caching</rdfs:label>
    <rdfs:comment>Negative caching allows per-status code TTLs to be set, in order to apply fine-grained caching for common errors or redirects.</rdfs:comment>
    <rdfs:domain rdf:resource="http://example.org/onto/class/google_compute_backend_bucket"/>
    <rdfs:range rdf:resource="http://www.w3.org/2001/XMLSchema#string"/>
  </owl:DatatypeProperty>
  <owl:DatatypeProperty rdf:about="http://example.org/onto/prop/google_compute_backend_bucket_request_coalescing">
    <rdfs:label>request_coalescing</rdfs:label>
    <rdfs:comment>If true then Cloud CDN will combine multiple concurrent cache fill requests into a small number of requests to the origin.</rdfs:comment>
    <rdfs:domain rdf:resource="http://example.org/onto/class/google_compute_backend_bucket"/>
    <rdfs:range rdf:resource="http://www.w3.org/2001/XMLSchema#string"/>
  </owl:DatatypeProperty>
  <owl:DatatypeProperty rdf:about="http://example.org/onto/prop/google_compute_backend_bucket_serve_while_stale">
    <rdfs:label>serve_while_stale</rdfs:label>
    <rdfs:comment>Serve existing content from the cache (if available) when revalidating content with the origin, or when an error is encountered when refreshing the cache.</rdfs:comment>
    <rdfs:domain rdf:resource="http://example.org/onto/class/google_compute_backend_bucket"/>
    <rdfs:range rdf:resource="http://www.w3.org/2001/XMLSchema#string"/>
  </owl:DatatypeProperty>
  <owl:DatatypeProperty rdf:about="http://example.org/onto/prop/google_compute_backend_bucket_signed_url_cache_max_age_sec">
    <rdfs:label>signed_url_cache_max_age_sec</rdfs:label>
    <rdfs:comment>Maximum number of seconds the response to a signed URL request will
be considered fresh. After this time period,
the response will be revalidated before being served.
When serving responses to signed URL requests,
Cloud CDN will internally behave as though
all responses from this backend had a "Cache-Control: public,
max-age=[TTL]" header, regardless of any existing Cache-Control
header. The actual headers served in responses will not be altered.</rdfs:comment>
    <rdfs:domain rdf:resource="http://example.org/onto/class/google_compute_backend_bucket"/>
    <rdfs:range rdf:resource="http://www.w3.org/2001/XMLSchema#string"/>
  </owl:DatatypeProperty>
  <owl:DatatypeProperty rdf:about="http://example.org/onto/prop/google_compute_backend_bucket_header_name">
    <rdfs:label>header_name</rdfs:label>
    <rdfs:comment>The header field name to match on when bypassing cache. Values are case-insensitive.</rdfs:comment>
    <rdfs:domain rdf:resource="http://example.org/onto/class/google_compute_backend_bucket"/>
    <rdfs:range rdf:resource="http://www.w3.org/2001/XMLSchema#string"/>
  </owl:DatatypeProperty>
  <owl:DatatypeProperty rdf:about="http://example.org/onto/prop/google_compute_backend_bucket_include_http_headers">
    <rdfs:label>include_http_headers</rdfs:label>
    <rdfs:comment>Allows HTTP request headers (by name) to be used in the
cache key.</rdfs:comment>
    <rdfs:domain rdf:resource="http://example.org/onto/class/google_compute_backend_bucket"/>
    <rdfs:range rdf:resource="http://www.w3.org/2001/XMLSchema#string"/>
  </owl:DatatypeProperty>
  <owl:DatatypeProperty rdf:about="http://example.org/onto/prop/google_compute_backend_bucket_query_string_whitelist">
    <rdfs:label>query_string_whitelist</rdfs:label>
    <rdfs:comment>Names of query string parameters to include in cache keys.
Default parameters are always included. '&' and '=' will
be percent encoded and not treated as delimiters.</rdfs:comment>
    <rdfs:domain rdf:resource="http://example.org/onto/class/google_compute_backend_bucket"/>
    <rdfs:range rdf:resource="http://www.w3.org/2001/XMLSchema#string"/>
  </owl:DatatypeProperty>
  <owl:DatatypeProperty rdf:about="http://example.org/onto/prop/google_compute_backend_bucket_code">
    <rdfs:label>code</rdfs:label>
    <rdfs:comment>The HTTP status code to define a TTL against. Only HTTP status codes 300, 301, 308, 404, 405, 410, 421, 451 and 501
can be specified as values, and you cannot specify a status code more than once.</rdfs:comment>
    <rdfs:domain rdf:resource="http://example.org/onto/class/google_compute_backend_bucket"/>
    <rdfs:range rdf:resource="http://www.w3.org/2001/XMLSchema#string"/>
  </owl:DatatypeProperty>
  <owl:DatatypeProperty rdf:about="http://example.org/onto/prop/google_compute_backend_bucket_ttl">
    <rdfs:label>ttl</rdfs:label>
    <rdfs:comment>The TTL (in seconds) for which to cache responses with the corresponding status code. The maximum allowed value is 1800s
(30 minutes), noting that infrequently accessed objects may be evicted from the cache before the defined TTL.</rdfs:comment>
    <rdfs:domain rdf:resource="http://example.org/onto/class/google_compute_backend_bucket"/>
    <rdfs:range rdf:resource="http://www.w3.org/2001/XMLSchema#string"/>
  </owl:DatatypeProperty>
  <owl:DatatypeProperty rdf:about="http://example.org/onto/prop/google_compute_backend_bucket_resource_manager_tags">
    <rdfs:label>resource_manager_tags</rdfs:label>
    <rdfs:comment>Resource manager tags to be bound to the backend bucket. Tag keys and values have the
same definition as resource manager tags. Keys must be in the format tagKeys/{tag_key_id},
and values are in the format tagValues/456.</rdfs:comment>
    <rdfs:domain rdf:resource="http://example.org/onto/class/google_compute_backend_bucket"/>
    <rdfs:range rdf:resource="http://www.w3.org/2001/XMLSchema#string"/>
  </owl:DatatypeProperty>
  <owl:DatatypeProperty rdf:about="http://example.org/onto/prop/google_compute_backend_bucket_create">
    <rdfs:label>create</rdfs:label>
    <rdfs:domain rdf:resource="http://example.org/onto/class/google_compute_backend_bucket"/>
    <rdfs:range rdf:resource="http://www.w3.org/2001/XMLSchema#string"/>
  </owl:DatatypeProperty>
  <owl:DatatypeProperty rdf:about="http://example.org/onto/prop/google_compute_backend_bucket_delete">
    <rdfs:label>delete</rdfs:label>
    <rdfs:domain rdf:resource="http://example.org/onto/class/google_compute_backend_bucket"/>
    <rdfs:range rdf:resource="http://www.w3.org/2001/XMLSchema#string"/>
  </owl:DatatypeProperty>
  <owl:DatatypeProperty rdf:about="http://example.org/onto/prop/google_compute_backend_bucket_update">
    <rdfs:label>update</rdfs:label>
    <rdfs:domain rdf:resource="http://example.org/onto/class/google_compute_backend_bucket"/>
    <rdfs:range rdf:resource="http://www.w3.org/2001/XMLSchema#string"/>
  </owl:DatatypeProperty>
</rdf:RDF>
