<?xml version="1.0" encoding="UTF-8"?>
<rdf:RDF
  xmlns:rdf="http://www.w3.org/1999/02/22-rdf-syntax-ns#"
  xmlns:rdfs="http://www.w3.org/2000/01/rdf-schema#"
  xmlns:owl="http://www.w3.org/2002/07/owl#"
  xmlns:xsd="http://www.w3.org/2001/XMLSchema#"
  xml:base="http://example.org/onto/">
  <owl:Class rdf:about="http://example.org/onto/class/google_compute_firewall_policy_rule">
    <rdfs:label>google_compute_firewall_policy_rule</rdfs:label>
    <rdfs:comment>#
#     ***     AUTO GENERATED CODE    ***    Type: MMv1     ***
#
# ----------------------------------------------------------------------------
#
#     This code is generated by Magic Modules using the following:
#
#     Configuration: https:#github.com/GoogleCloudPlatform/magic-modules/tree/main/mmv1/products/compute/FirewallPolicyRule.yaml
#     Template:      https:#github.com/GoogleCloudPlatform/magic-modules/tree/main/mmv1/templates/terraform/resource.html.markdown.tmpl
#
#     DO NOT EDIT this file directly. Any changes made to this file will be
#     overwritten during the next generation cycle.
#
# ----------------------------------------------------------------------------
subcategory: "Compute Engine"
description: |-
  Represents a rule that describes one or more match conditions along with the action to be taken when traffic matches this condition (allow or deny).
---</rdfs:comment>
  </owl:Class>
  <owl:DatatypeProperty rdf:about="http://example.org/onto/prop/google_compute_firewall_policy_rule_action">
    <rdfs:label>action</rdfs:label>
    <rdfs:comment>The Action to perform when the client connection triggers the rule. Valid actions are "allow", "deny", "goto_next" and "apply_security_profile_group".</rdfs:comment>
    <rdfs:domain rdf:resource="http://example.org/onto/class/google_compute_firewall_policy_rule"/>
    <rdfs:range rdf:resource="http://www.w3.org/2001/XMLSchema#string"/>
  </owl:DatatypeProperty>
  <owl:DatatypeProperty rdf:about="http://example.org/onto/prop/google_compute_firewall_policy_rule_creation_timestamp">
    <rdfs:label>creation_timestamp</rdfs:label>
    <rdfs:comment>Creation timestamp in RFC3339 text format.</rdfs:comment>
    <rdfs:domain rdf:resource="http://example.org/onto/class/google_compute_firewall_policy_rule"/>
    <rdfs:range rdf:resource="http://www.w3.org/2001/XMLSchema#string"/>
  </owl:DatatypeProperty>
  <owl:DatatypeProperty rdf:about="http://example.org/onto/prop/google_compute_firewall_policy_rule_description">
    <rdfs:label>description</rdfs:label>
    <rdfs:comment>An optional description for this resource.</rdfs:comment>
    <rdfs:domain rdf:resource="http://example.org/onto/class/google_compute_firewall_policy_rule"/>
    <rdfs:range rdf:resource="http://www.w3.org/2001/XMLSchema#string"/>
  </owl:DatatypeProperty>
  <owl:DatatypeProperty rdf:about="http://example.org/onto/prop/google_compute_firewall_policy_rule_direction">
    <rdfs:label>direction</rdfs:label>
    <rdfs:comment>The direction in which this rule applies. Possible values: ["INGRESS", "EGRESS"]</rdfs:comment>
    <rdfs:domain rdf:resource="http://example.org/onto/class/google_compute_firewall_policy_rule"/>
    <rdfs:range rdf:resource="http://www.w3.org/2001/XMLSchema#string"/>
  </owl:DatatypeProperty>
  <owl:DatatypeProperty rdf:about="http://example.org/onto/prop/google_compute_firewall_policy_rule_disabled">
    <rdfs:label>disabled</rdfs:label>
    <rdfs:comment>Denotes whether the firewall policy rule is disabled.
When set to true, the firewall policy rule is not enforced and traffic behaves as if it did not exist.
If this is unspecified, the firewall policy rule will be enabled.</rdfs:comment>
    <rdfs:domain rdf:resource="http://example.org/onto/class/google_compute_firewall_policy_rule"/>
    <rdfs:range rdf:resource="http://www.w3.org/2001/XMLSchema#string"/>
  </owl:DatatypeProperty>
  <owl:DatatypeProperty rdf:about="http://example.org/onto/prop/google_compute_firewall_policy_rule_enable_logging">
    <rdfs:label>enable_logging</rdfs:label>
    <rdfs:comment>Denotes whether to enable logging for a particular rule.
If logging is enabled, logs will be exported to the configured export destination in Stackdriver.
Logs may be exported to BigQuery or Pub/Sub.
Note: you cannot enable logging on "goto_next" rules.</rdfs:comment>
    <rdfs:domain rdf:resource="http://example.org/onto/class/google_compute_firewall_policy_rule"/>
    <rdfs:range rdf:resource="http://www.w3.org/2001/XMLSchema#string"/>
  </owl:DatatypeProperty>
  <owl:DatatypeProperty rdf:about="http://example.org/onto/prop/google_compute_firewall_policy_rule_firewall_policy">
    <rdfs:label>firewall_policy</rdfs:label>
    <rdfs:comment>The firewall policy of the resource.</rdfs:comment>
    <rdfs:domain rdf:resource="http://example.org/onto/class/google_compute_firewall_policy_rule"/>
    <rdfs:range rdf:resource="http://www.w3.org/2001/XMLSchema#string"/>
  </owl:DatatypeProperty>
  <owl:DatatypeProperty rdf:about="http://example.org/onto/prop/google_compute_firewall_policy_rule_id">
    <rdfs:label>id</rdfs:label>
    <rdfs:domain rdf:resource="http://example.org/onto/class/google_compute_firewall_policy_rule"/>
    <rdfs:range rdf:resource="http://www.w3.org/2001/XMLSchema#string"/>
  </owl:DatatypeProperty>
  <owl:DatatypeProperty rdf:about="http://example.org/onto/prop/google_compute_firewall_policy_rule_kind">
    <rdfs:label>kind</rdfs:label>
    <rdfs:comment>Type of the resource. Always 'compute#firewallPolicyRule' for firewall policy rules</rdfs:comment>
    <rdfs:domain rdf:resource="http://example.org/onto/class/google_compute_firewall_policy_rule"/>
    <rdfs:range rdf:resource="http://www.w3.org/2001/XMLSchema#string"/>
  </owl:DatatypeProperty>
  <owl:DatatypeProperty rdf:about="http://example.org/onto/prop/google_compute_firewall_policy_rule_priority">
    <rdfs:label>priority</rdfs:label>
    <rdfs:comment>An integer indicating the priority of a rule in the list.
The priority must be a positive value between 0 and 2147483647.
Rules are evaluated from highest to lowest priority where 0 is the highest priority and 2147483647 is the lowest prority.</rdfs:comment>
    <rdfs:domain rdf:resource="http://example.org/onto/class/google_compute_firewall_policy_rule"/>
    <rdfs:range rdf:resource="http://www.w3.org/2001/XMLSchema#string"/>
  </owl:DatatypeProperty>
  <owl:DatatypeProperty rdf:about="http://example.org/onto/prop/google_compute_firewall_policy_rule_rule_tuple_count">
    <rdfs:label>rule_tuple_count</rdfs:label>
    <rdfs:comment>Calculation of the complexity of a single firewall policy rule.</rdfs:comment>
    <rdfs:domain rdf:resource="http://example.org/onto/class/google_compute_firewall_policy_rule"/>
    <rdfs:range rdf:resource="http://www.w3.org/2001/XMLSchema#string"/>
  </owl:DatatypeProperty>
  <owl:DatatypeProperty rdf:about="http://example.org/onto/prop/google_compute_firewall_policy_rule_security_profile_group">
    <rdfs:label>security_profile_group</rdfs:label>
    <rdfs:comment>A fully-qualified URL of a SecurityProfile resource instance.
Example: https://networksecurity.googleapis.com/v1/projects/{project}/locations/{location}/securityProfileGroups/my-security-profile-group
Must be specified if action = 'apply_security_profile_group' and cannot be specified for other actions.</rdfs:comment>
    <rdfs:domain rdf:resource="http://example.org/onto/class/google_compute_firewall_policy_rule"/>
    <rdfs:range rdf:resource="http://www.w3.org/2001/XMLSchema#string"/>
  </owl:DatatypeProperty>
  <owl:DatatypeProperty rdf:about="http://example.org/onto/prop/google_compute_firewall_policy_rule_target_resources">
    <rdfs:label>target_resources</rdfs:label>
    <rdfs:comment>A list of network resource URLs to which this rule applies.
This field allows you to control which network's VMs get this rule.
If this field is left blank, all VMs within the organization will receive the rule.</rdfs:comment>
    <rdfs:domain rdf:resource="http://example.org/onto/class/google_compute_firewall_policy_rule"/>
    <rdfs:range rdf:resource="http://www.w3.org/2001/XMLSchema#string"/>
  </owl:DatatypeProperty>
  <owl:DatatypeProperty rdf:about="http://example.org/onto/prop/google_compute_firewall_policy_rule_target_service_accounts">
    <rdfs:label>target_service_accounts</rdfs:label>
    <rdfs:comment>A list of service accounts indicating the sets of instances that are applied with this rule.</rdfs:comment>
    <rdfs:domain rdf:resource="http://example.org/onto/class/google_compute_firewall_policy_rule"/>
    <rdfs:range rdf:resource="http://www.w3.org/2001/XMLSchema#string"/>
  </owl:DatatypeProperty>
  <owl:DatatypeProperty rdf:about="http://example.org/onto/prop/google_compute_firewall_policy_rule_tls_inspect">
    <rdfs:label>tls_inspect</rdfs:label>
    <rdfs:comment>Boolean flag indicating if the traffic should be TLS decrypted.
Can be set only if action = 'apply_security_profile_group' and cannot be set for other actions.</rdfs:comment>
    <rdfs:domain rdf:resource="http://example.org/onto/class/google_compute_firewall_policy_rule"/>
    <rdfs:range rdf:resource="http://www.w3.org/2001/XMLSchema#string"/>
  </owl:DatatypeProperty>
  <owl:DatatypeProperty rdf:about="http://example.org/onto/prop/google_compute_firewall_policy_rule_dest_address_groups">
    <rdfs:label>dest_address_groups</rdfs:label>
    <rdfs:comment>Address groups which should be matched against the traffic destination. Maximum number of destination address groups is 10.</rdfs:comment>
    <rdfs:domain rdf:resource="http://example.org/onto/class/google_compute_firewall_policy_rule"/>
    <rdfs:range rdf:resource="http://www.w3.org/2001/XMLSchema#string"/>
  </owl:DatatypeProperty>
  <owl:DatatypeProperty rdf:about="http://example.org/onto/prop/google_compute_firewall_policy_rule_dest_fqdns">
    <rdfs:label>dest_fqdns</rdfs:label>
    <rdfs:comment>Fully Qualified Domain Name (FQDN) which should be matched against traffic destination. Maximum number of destination fqdn allowed is 100.</rdfs:comment>
    <rdfs:domain rdf:resource="http://example.org/onto/class/google_compute_firewall_policy_rule"/>
    <rdfs:range rdf:resource="http://www.w3.org/2001/XMLSchema#string"/>
  </owl:DatatypeProperty>
  <owl:DatatypeProperty rdf:about="http://example.org/onto/prop/google_compute_firewall_policy_rule_dest_ip_ranges">
    <rdfs:label>dest_ip_ranges</rdfs:label>
    <rdfs:comment>CIDR IP address range. Maximum number of destination CIDR IP ranges allowed is 5000.</rdfs:comment>
    <rdfs:domain rdf:resource="http://example.org/onto/class/google_compute_firewall_policy_rule"/>
    <rdfs:range rdf:resource="http://www.w3.org/2001/XMLSchema#string"/>
  </owl:DatatypeProperty>
  <owl:DatatypeProperty rdf:about="http://example.org/onto/prop/google_compute_firewall_policy_rule_dest_region_codes">
    <rdfs:label>dest_region_codes</rdfs:label>
    <rdfs:comment>Region codes whose IP addresses will be used to match for destination of traffic. Should be specified as 2 letter country code defined as per ISO 3166 alpha-2 country codes. ex."US" Maximum number of dest region codes allowed is 5000.</rdfs:comment>
    <rdfs:domain rdf:resource="http://example.org/onto/class/google_compute_firewall_policy_rule"/>
    <rdfs:range rdf:resource="http://www.w3.org/2001/XMLSchema#string"/>
  </owl:DatatypeProperty>
  <owl:DatatypeProperty rdf:about="http://example.org/onto/prop/google_compute_firewall_policy_rule_dest_threat_intelligences">
    <rdfs:label>dest_threat_intelligences</rdfs:label>
    <rdfs:comment>Names of Network Threat Intelligence lists. The IPs in these lists will be matched against traffic destination.</rdfs:comment>
    <rdfs:domain rdf:resource="http://example.org/onto/class/google_compute_firewall_policy_rule"/>
    <rdfs:range rdf:resource="http://www.w3.org/2001/XMLSchema#string"/>
  </owl:DatatypeProperty>
  <owl:DatatypeProperty rdf:about="http://example.org/onto/prop/google_compute_firewall_policy_rule_src_address_groups">
    <rdfs:label>src_address_groups</rdfs:label>
    <rdfs:comment>Address groups which should be matched against the traffic source. Maximum number of source address groups is 10.</rdfs:comment>
    <rdfs:domain rdf:resource="http://example.org/onto/class/google_compute_firewall_policy_rule"/>
    <rdfs:range rdf:resource="http://www.w3.org/2001/XMLSchema#string"/>
  </owl:DatatypeProperty>
  <owl:DatatypeProperty rdf:about="http://example.org/onto/prop/google_compute_firewall_policy_rule_src_fqdns">
    <rdfs:label>src_fqdns</rdfs:label>
    <rdfs:comment>Fully Qualified Domain Name (FQDN) which should be matched against traffic source. Maximum number of source fqdn allowed is 100.</rdfs:comment>
    <rdfs:domain rdf:resource="http://example.org/onto/class/google_compute_firewall_policy_rule"/>
    <rdfs:range rdf:resource="http://www.w3.org/2001/XMLSchema#string"/>
  </owl:DatatypeProperty>
  <owl:DatatypeProperty rdf:about="http://example.org/onto/prop/google_compute_firewall_policy_rule_src_ip_ranges">
    <rdfs:label>src_ip_ranges</rdfs:label>
    <rdfs:comment>CIDR IP address range. Maximum number of source CIDR IP ranges allowed is 5000.</rdfs:comment>
    <rdfs:domain rdf:resource="http://example.org/onto/class/google_compute_firewall_policy_rule"/>
    <rdfs:range rdf:resource="http://www.w3.org/2001/XMLSchema#string"/>
  </owl:DatatypeProperty>
  <owl:DatatypeProperty rdf:about="http://example.org/onto/prop/google_compute_firewall_policy_rule_src_region_codes">
    <rdfs:label>src_region_codes</rdfs:label>
    <rdfs:comment>Region codes whose IP addresses will be used to match for source of traffic. Should be specified as 2 letter country code defined as per ISO 3166 alpha-2 country codes. ex."US" Maximum number of source region codes allowed is 5000.</rdfs:comment>
    <rdfs:domain rdf:resource="http://example.org/onto/class/google_compute_firewall_policy_rule"/>
    <rdfs:range rdf:resource="http://www.w3.org/2001/XMLSchema#string"/>
  </owl:DatatypeProperty>
  <owl:DatatypeProperty rdf:about="http://example.org/onto/prop/google_compute_firewall_policy_rule_src_threat_intelligences">
    <rdfs:label>src_threat_intelligences</rdfs:label>
    <rdfs:comment>Names of Network Threat Intelligence lists. The IPs in these lists will be matched against traffic source.</rdfs:comment>
    <rdfs:domain rdf:resource="http://example.org/onto/class/google_compute_firewall_policy_rule"/>
    <rdfs:range rdf:resource="http://www.w3.org/2001/XMLSchema#string"/>
  </owl:DatatypeProperty>
  <owl:DatatypeProperty rdf:about="http://example.org/onto/prop/google_compute_firewall_policy_rule_ip_protocol">
    <rdfs:label>ip_protocol</rdfs:label>
    <rdfs:comment>The IP protocol to which this rule applies. The protocol type is required when creating a firewall rule.
This value can either be one of the following well known protocol strings (tcp, udp, icmp, esp, ah, ipip, sctp), or the IP protocol number.</rdfs:comment>
    <rdfs:domain rdf:resource="http://example.org/onto/class/google_compute_firewall_policy_rule"/>
    <rdfs:range rdf:resource="http://www.w3.org/2001/XMLSchema#string"/>
  </owl:DatatypeProperty>
  <owl:DatatypeProperty rdf:about="http://example.org/onto/prop/google_compute_firewall_policy_rule_ports">
    <rdfs:label>ports</rdfs:label>
    <rdfs:comment>An optional list of ports to which this rule applies. This field is only applicable for UDP or TCP protocol. Each entry must be either an integer or a range. If not specified, this rule applies to connections through any port.
Example inputs include: ["22"], ["80","443"], and ["12345-12349"].</rdfs:comment>
    <rdfs:domain rdf:resource="http://example.org/onto/class/google_compute_firewall_policy_rule"/>
    <rdfs:range rdf:resource="http://www.w3.org/2001/XMLSchema#string"/>
  </owl:DatatypeProperty>
  <owl:DatatypeProperty rdf:about="http://example.org/onto/prop/google_compute_firewall_policy_rule_name">
    <rdfs:label>name</rdfs:label>
    <rdfs:comment>Name of the secure tag, created with TagManager's TagValue API.</rdfs:comment>
    <rdfs:domain rdf:resource="http://example.org/onto/class/google_compute_firewall_policy_rule"/>
    <rdfs:range rdf:resource="http://www.w3.org/2001/XMLSchema#string"/>
  </owl:DatatypeProperty>
  <owl:DatatypeProperty rdf:about="http://example.org/onto/prop/google_compute_firewall_policy_rule_state">
    <rdfs:label>state</rdfs:label>
    <rdfs:comment>State of the secure tag, either EFFECTIVE or INEFFECTIVE. A secure tag is INEFFECTIVE when it is deleted or its network is deleted.</rdfs:comment>
    <rdfs:domain rdf:resource="http://example.org/onto/class/google_compute_firewall_policy_rule"/>
    <rdfs:range rdf:resource="http://www.w3.org/2001/XMLSchema#string"/>
  </owl:DatatypeProperty>
  <owl:DatatypeProperty rdf:about="http://example.org/onto/prop/google_compute_firewall_policy_rule_name">
    <rdfs:label>name</rdfs:label>
    <rdfs:comment>Name of the secure tag, created with TagManager's TagValue API.</rdfs:comment>
    <rdfs:domain rdf:resource="http://example.org/onto/class/google_compute_firewall_policy_rule"/>
    <rdfs:range rdf:resource="http://www.w3.org/2001/XMLSchema#string"/>
  </owl:DatatypeProperty>
  <owl:DatatypeProperty rdf:about="http://example.org/onto/prop/google_compute_firewall_policy_rule_state">
    <rdfs:label>state</rdfs:label>
    <rdfs:comment>State of the secure tag, either EFFECTIVE or INEFFECTIVE. A secure tag is INEFFECTIVE when it is deleted or its network is deleted.</rdfs:comment>
    <rdfs:domain rdf:resource="http://example.org/onto/class/google_compute_firewall_policy_rule"/>
    <rdfs:range rdf:resource="http://www.w3.org/2001/XMLSchema#string"/>
  </owl:DatatypeProperty>
  <owl:DatatypeProperty rdf:about="http://example.org/onto/prop/google_compute_firewall_policy_rule_create">
    <rdfs:label>create</rdfs:label>
    <rdfs:domain rdf:resource="http://example.org/onto/class/google_compute_firewall_policy_rule"/>
    <rdfs:range rdf:resource="http://www.w3.org/2001/XMLSchema#string"/>
  </owl:DatatypeProperty>
  <owl:DatatypeProperty rdf:about="http://example.org/onto/prop/google_compute_firewall_policy_rule_delete">
    <rdfs:label>delete</rdfs:label>
    <rdfs:domain rdf:resource="http://example.org/onto/class/google_compute_firewall_policy_rule"/>
    <rdfs:range rdf:resource="http://www.w3.org/2001/XMLSchema#string"/>
  </owl:DatatypeProperty>
  <owl:DatatypeProperty rdf:about="http://example.org/onto/prop/google_compute_firewall_policy_rule_update">
    <rdfs:label>update</rdfs:label>
    <rdfs:domain rdf:resource="http://example.org/onto/class/google_compute_firewall_policy_rule"/>
    <rdfs:range rdf:resource="http://www.w3.org/2001/XMLSchema#string"/>
  </owl:DatatypeProperty>
</rdf:RDF>
