<?xml version="1.0" encoding="UTF-8"?>
<rdf:RDF
  xmlns:rdf="http://www.w3.org/1999/02/22-rdf-syntax-ns#"
  xmlns:rdfs="http://www.w3.org/2000/01/rdf-schema#"
  xmlns:owl="http://www.w3.org/2002/07/owl#"
  xmlns:xsd="http://www.w3.org/2001/XMLSchema#"
  xml:base="http://example.org/onto/">
  <owl:Class rdf:about="http://example.org/onto/class/google_apihub_plugin_instance">
    <rdfs:label>google_apihub_plugin_instance</rdfs:label>
    <rdfs:comment>#
#     ***     AUTO GENERATED CODE    ***    Type: MMv1     ***
#
# ----------------------------------------------------------------------------
#
#     This code is generated by Magic Modules using the following:
#
#     Configuration: https:#github.com/GoogleCloudPlatform/magic-modules/tree/main/mmv1/products/apihub/PluginInstance.yaml
#     Template:      https:#github.com/GoogleCloudPlatform/magic-modules/tree/main/mmv1/templates/terraform/resource.html.markdown.tmpl
#
#     DO NOT EDIT this file directly. Any changes made to this file will be
#     overwritten during the next generation cycle.
#
# ----------------------------------------------------------------------------
subcategory: "API Hub"
description: |-
  Description
---</rdfs:comment>
  </owl:Class>
  <owl:DatatypeProperty rdf:about="http://example.org/onto/prop/google_apihub_plugin_instance_create_time">
    <rdfs:label>create_time</rdfs:label>
    <rdfs:comment>Timestamp indicating when the plugin instance was created.</rdfs:comment>
    <rdfs:domain rdf:resource="http://example.org/onto/class/google_apihub_plugin_instance"/>
    <rdfs:range rdf:resource="http://www.w3.org/2001/XMLSchema#string"/>
  </owl:DatatypeProperty>
  <owl:DatatypeProperty rdf:about="http://example.org/onto/prop/google_apihub_plugin_instance_disable">
    <rdfs:label>disable</rdfs:label>
    <rdfs:comment>The display name for this plugin instance. Max length is 255 characters.</rdfs:comment>
    <rdfs:domain rdf:resource="http://example.org/onto/class/google_apihub_plugin_instance"/>
    <rdfs:range rdf:resource="http://www.w3.org/2001/XMLSchema#string"/>
  </owl:DatatypeProperty>
  <owl:DatatypeProperty rdf:about="http://example.org/onto/prop/google_apihub_plugin_instance_display_name">
    <rdfs:label>display_name</rdfs:label>
    <rdfs:comment>The display name for this plugin instance. Max length is 255 characters.</rdfs:comment>
    <rdfs:domain rdf:resource="http://example.org/onto/class/google_apihub_plugin_instance"/>
    <rdfs:range rdf:resource="http://www.w3.org/2001/XMLSchema#string"/>
  </owl:DatatypeProperty>
  <owl:DatatypeProperty rdf:about="http://example.org/onto/prop/google_apihub_plugin_instance_error_message">
    <rdfs:label>error_message</rdfs:label>
    <rdfs:comment>Error message describing the failure, if any, during Create, Delete or
ApplyConfig operation corresponding to the plugin instance.This field will
only be populated if the plugin instance is in the ERROR or FAILED state.</rdfs:comment>
    <rdfs:domain rdf:resource="http://example.org/onto/class/google_apihub_plugin_instance"/>
    <rdfs:range rdf:resource="http://www.w3.org/2001/XMLSchema#string"/>
  </owl:DatatypeProperty>
  <owl:DatatypeProperty rdf:about="http://example.org/onto/prop/google_apihub_plugin_instance_id">
    <rdfs:label>id</rdfs:label>
    <rdfs:domain rdf:resource="http://example.org/onto/class/google_apihub_plugin_instance"/>
    <rdfs:range rdf:resource="http://www.w3.org/2001/XMLSchema#string"/>
  </owl:DatatypeProperty>
  <owl:DatatypeProperty rdf:about="http://example.org/onto/prop/google_apihub_plugin_instance_location">
    <rdfs:label>location</rdfs:label>
    <rdfs:comment>Resource ID segment making up resource 'name'. It identifies the resource within its parent collection as described in https://google.aip.dev/122.</rdfs:comment>
    <rdfs:domain rdf:resource="http://example.org/onto/class/google_apihub_plugin_instance"/>
    <rdfs:range rdf:resource="http://www.w3.org/2001/XMLSchema#string"/>
  </owl:DatatypeProperty>
  <owl:DatatypeProperty rdf:about="http://example.org/onto/prop/google_apihub_plugin_instance_name">
    <rdfs:label>name</rdfs:label>
    <rdfs:comment>Identifier. The unique name of the plugin instance resource.
Format:
'projects/{project}/locations/{location}/plugins/{plugin}/instances/{instance}'</rdfs:comment>
    <rdfs:domain rdf:resource="http://example.org/onto/class/google_apihub_plugin_instance"/>
    <rdfs:range rdf:resource="http://www.w3.org/2001/XMLSchema#string"/>
  </owl:DatatypeProperty>
  <owl:DatatypeProperty rdf:about="http://example.org/onto/prop/google_apihub_plugin_instance_plugin">
    <rdfs:label>plugin</rdfs:label>
    <rdfs:comment>Resource ID segment making up resource 'name'. It identifies the resource within its parent collection as described in https://google.aip.dev/122.</rdfs:comment>
    <rdfs:domain rdf:resource="http://example.org/onto/class/google_apihub_plugin_instance"/>
    <rdfs:range rdf:resource="http://www.w3.org/2001/XMLSchema#string"/>
  </owl:DatatypeProperty>
  <owl:DatatypeProperty rdf:about="http://example.org/onto/prop/google_apihub_plugin_instance_plugin_instance_id">
    <rdfs:label>plugin_instance_id</rdfs:label>
    <rdfs:comment>The ID to use for the plugin instance, which will become the final
component of the plugin instance's resource name. This field is optional.

* If provided, the same will be used. The service will throw an error if
the specified id is already used by another plugin instance in the plugin
resource.
* If not provided, a system generated id will be used.

This value should be 4-63 characters, and valid characters
are /a-z[0-9]-_/.</rdfs:comment>
    <rdfs:domain rdf:resource="http://example.org/onto/class/google_apihub_plugin_instance"/>
    <rdfs:range rdf:resource="http://www.w3.org/2001/XMLSchema#string"/>
  </owl:DatatypeProperty>
  <owl:DatatypeProperty rdf:about="http://example.org/onto/prop/google_apihub_plugin_instance_project">
    <rdfs:label>project</rdfs:label>
    <rdfs:domain rdf:resource="http://example.org/onto/class/google_apihub_plugin_instance"/>
    <rdfs:range rdf:resource="http://www.w3.org/2001/XMLSchema#string"/>
  </owl:DatatypeProperty>
  <owl:DatatypeProperty rdf:about="http://example.org/onto/prop/google_apihub_plugin_instance_state">
    <rdfs:label>state</rdfs:label>
    <rdfs:comment>The current state of the plugin instance (e.g., enabled, disabled,
provisioning).
Possible values:
STATE_UNSPECIFIED
CREATING
ACTIVE
APPLYING_CONFIG
ERROR
FAILED
DELETING</rdfs:comment>
    <rdfs:domain rdf:resource="http://example.org/onto/class/google_apihub_plugin_instance"/>
    <rdfs:range rdf:resource="http://www.w3.org/2001/XMLSchema#string"/>
  </owl:DatatypeProperty>
  <owl:DatatypeProperty rdf:about="http://example.org/onto/prop/google_apihub_plugin_instance_update_time">
    <rdfs:label>update_time</rdfs:label>
    <rdfs:comment>Timestamp indicating when the plugin instance was last updated.</rdfs:comment>
    <rdfs:domain rdf:resource="http://example.org/onto/class/google_apihub_plugin_instance"/>
    <rdfs:range rdf:resource="http://www.w3.org/2001/XMLSchema#string"/>
  </owl:DatatypeProperty>
  <owl:DatatypeProperty rdf:about="http://example.org/onto/prop/google_apihub_plugin_instance_action_id">
    <rdfs:label>action_id</rdfs:label>
    <rdfs:comment>This should map to one of the action id specified
in actions_config in the plugin.</rdfs:comment>
    <rdfs:domain rdf:resource="http://example.org/onto/class/google_apihub_plugin_instance"/>
    <rdfs:range rdf:resource="http://www.w3.org/2001/XMLSchema#string"/>
  </owl:DatatypeProperty>
  <owl:DatatypeProperty rdf:about="http://example.org/onto/prop/google_apihub_plugin_instance_hub_instance_action">
    <rdfs:label>hub_instance_action</rdfs:label>
    <rdfs:comment>The execution status for the plugin instance.</rdfs:comment>
    <rdfs:domain rdf:resource="http://example.org/onto/class/google_apihub_plugin_instance"/>
    <rdfs:range rdf:resource="http://www.w3.org/2001/XMLSchema#string"/>
  </owl:DatatypeProperty>
  <owl:DatatypeProperty rdf:about="http://example.org/onto/prop/google_apihub_plugin_instance_schedule_cron_expression">
    <rdfs:label>schedule_cron_expression</rdfs:label>
    <rdfs:comment>The schedule for this plugin instance action. This can only be set if the
plugin supports API_HUB_SCHEDULE_TRIGGER mode for this action.</rdfs:comment>
    <rdfs:domain rdf:resource="http://example.org/onto/class/google_apihub_plugin_instance"/>
    <rdfs:range rdf:resource="http://www.w3.org/2001/XMLSchema#string"/>
  </owl:DatatypeProperty>
  <owl:DatatypeProperty rdf:about="http://example.org/onto/prop/google_apihub_plugin_instance_schedule_time_zone">
    <rdfs:label>schedule_time_zone</rdfs:label>
    <rdfs:comment>The time zone for the schedule cron expression. If not provided, UTC will
be used.</rdfs:comment>
    <rdfs:domain rdf:resource="http://example.org/onto/class/google_apihub_plugin_instance"/>
    <rdfs:range rdf:resource="http://www.w3.org/2001/XMLSchema#string"/>
  </owl:DatatypeProperty>
  <owl:DatatypeProperty rdf:about="http://example.org/onto/prop/google_apihub_plugin_instance_state">
    <rdfs:label>state</rdfs:label>
    <rdfs:comment>The current state of the plugin action in the plugin instance.
Possible values:
STATE_UNSPECIFIED
ENABLED
DISABLED
ENABLING
DISABLING
ERROR</rdfs:comment>
    <rdfs:domain rdf:resource="http://example.org/onto/class/google_apihub_plugin_instance"/>
    <rdfs:range rdf:resource="http://www.w3.org/2001/XMLSchema#string"/>
  </owl:DatatypeProperty>
  <owl:DatatypeProperty rdf:about="http://example.org/onto/prop/google_apihub_plugin_instance_curation_type">
    <rdfs:label>curation_type</rdfs:label>
    <rdfs:comment>Possible values:
CURATION_TYPE_UNSPECIFIED
DEFAULT_CURATION_FOR_API_METADATA
CUSTOM_CURATION_FOR_API_METADATA</rdfs:comment>
    <rdfs:domain rdf:resource="http://example.org/onto/class/google_apihub_plugin_instance"/>
    <rdfs:range rdf:resource="http://www.w3.org/2001/XMLSchema#string"/>
  </owl:DatatypeProperty>
  <owl:DatatypeProperty rdf:about="http://example.org/onto/prop/google_apihub_plugin_instance_curation">
    <rdfs:label>curation</rdfs:label>
    <rdfs:comment>The unique name of the curation resource. This will be the name of the
curation resource in the format:
'projects/{project}/locations/{location}/curations/{curation}'</rdfs:comment>
    <rdfs:domain rdf:resource="http://example.org/onto/class/google_apihub_plugin_instance"/>
    <rdfs:range rdf:resource="http://www.w3.org/2001/XMLSchema#string"/>
  </owl:DatatypeProperty>
  <owl:DatatypeProperty rdf:about="http://example.org/onto/prop/google_apihub_plugin_instance_auth_type">
    <rdfs:label>auth_type</rdfs:label>
    <rdfs:comment>Possible values:
AUTH_TYPE_UNSPECIFIED
NO_AUTH
GOOGLE_SERVICE_ACCOUNT
USER_PASSWORD
API_KEY
OAUTH2_CLIENT_CREDENTIALS</rdfs:comment>
    <rdfs:domain rdf:resource="http://example.org/onto/class/google_apihub_plugin_instance"/>
    <rdfs:range rdf:resource="http://www.w3.org/2001/XMLSchema#string"/>
  </owl:DatatypeProperty>
  <owl:DatatypeProperty rdf:about="http://example.org/onto/prop/google_apihub_plugin_instance_http_element_location">
    <rdfs:label>http_element_location</rdfs:label>
    <rdfs:comment>The location of the API key.
The default value is QUERY.
Possible values:
HTTP_ELEMENT_LOCATION_UNSPECIFIED
QUERY
HEADER
PATH
BODY
COOKIE</rdfs:comment>
    <rdfs:domain rdf:resource="http://example.org/onto/class/google_apihub_plugin_instance"/>
    <rdfs:range rdf:resource="http://www.w3.org/2001/XMLSchema#string"/>
  </owl:DatatypeProperty>
  <owl:DatatypeProperty rdf:about="http://example.org/onto/prop/google_apihub_plugin_instance_name">
    <rdfs:label>name</rdfs:label>
    <rdfs:comment>The parameter name of the API key.
E.g. If the API request is "https://example.com/act?api_key=",
"api_key" would be the parameter name.</rdfs:comment>
    <rdfs:domain rdf:resource="http://example.org/onto/class/google_apihub_plugin_instance"/>
    <rdfs:range rdf:resource="http://www.w3.org/2001/XMLSchema#string"/>
  </owl:DatatypeProperty>
  <owl:DatatypeProperty rdf:about="http://example.org/onto/prop/google_apihub_plugin_instance_secret_version">
    <rdfs:label>secret_version</rdfs:label>
    <rdfs:comment>The resource name of the secret version in the format,
format as: 'projects/*/secrets/*/versions/*'.</rdfs:comment>
    <rdfs:domain rdf:resource="http://example.org/onto/class/google_apihub_plugin_instance"/>
    <rdfs:range rdf:resource="http://www.w3.org/2001/XMLSchema#string"/>
  </owl:DatatypeProperty>
  <owl:DatatypeProperty rdf:about="http://example.org/onto/prop/google_apihub_plugin_instance_service_account">
    <rdfs:label>service_account</rdfs:label>
    <rdfs:comment>The service account to be used for authenticating request.

The 'iam.serviceAccounts.getAccessToken' permission should be granted on
this service account to the impersonator service account.</rdfs:comment>
    <rdfs:domain rdf:resource="http://example.org/onto/class/google_apihub_plugin_instance"/>
    <rdfs:range rdf:resource="http://www.w3.org/2001/XMLSchema#string"/>
  </owl:DatatypeProperty>
  <owl:DatatypeProperty rdf:about="http://example.org/onto/prop/google_apihub_plugin_instance_client_id">
    <rdfs:label>client_id</rdfs:label>
    <rdfs:comment>The client identifier.</rdfs:comment>
    <rdfs:domain rdf:resource="http://example.org/onto/class/google_apihub_plugin_instance"/>
    <rdfs:range rdf:resource="http://www.w3.org/2001/XMLSchema#string"/>
  </owl:DatatypeProperty>
  <owl:DatatypeProperty rdf:about="http://example.org/onto/prop/google_apihub_plugin_instance_secret_version">
    <rdfs:label>secret_version</rdfs:label>
    <rdfs:comment>The resource name of the secret version in the format,
format as: 'projects/*/secrets/*/versions/*'.</rdfs:comment>
    <rdfs:domain rdf:resource="http://example.org/onto/class/google_apihub_plugin_instance"/>
    <rdfs:range rdf:resource="http://www.w3.org/2001/XMLSchema#string"/>
  </owl:DatatypeProperty>
  <owl:DatatypeProperty rdf:about="http://example.org/onto/prop/google_apihub_plugin_instance_username">
    <rdfs:label>username</rdfs:label>
    <rdfs:comment>Username.</rdfs:comment>
    <rdfs:domain rdf:resource="http://example.org/onto/class/google_apihub_plugin_instance"/>
    <rdfs:range rdf:resource="http://www.w3.org/2001/XMLSchema#string"/>
  </owl:DatatypeProperty>
  <owl:DatatypeProperty rdf:about="http://example.org/onto/prop/google_apihub_plugin_instance_secret_version">
    <rdfs:label>secret_version</rdfs:label>
    <rdfs:comment>The resource name of the secret version in the format,
format as: 'projects/*/secrets/*/versions/*'.</rdfs:comment>
    <rdfs:domain rdf:resource="http://example.org/onto/class/google_apihub_plugin_instance"/>
    <rdfs:range rdf:resource="http://www.w3.org/2001/XMLSchema#string"/>
  </owl:DatatypeProperty>
  <owl:DatatypeProperty rdf:about="http://example.org/onto/prop/google_apihub_plugin_instance_create">
    <rdfs:label>create</rdfs:label>
    <rdfs:domain rdf:resource="http://example.org/onto/class/google_apihub_plugin_instance"/>
    <rdfs:range rdf:resource="http://www.w3.org/2001/XMLSchema#string"/>
  </owl:DatatypeProperty>
  <owl:DatatypeProperty rdf:about="http://example.org/onto/prop/google_apihub_plugin_instance_delete">
    <rdfs:label>delete</rdfs:label>
    <rdfs:domain rdf:resource="http://example.org/onto/class/google_apihub_plugin_instance"/>
    <rdfs:range rdf:resource="http://www.w3.org/2001/XMLSchema#string"/>
  </owl:DatatypeProperty>
  <owl:DatatypeProperty rdf:about="http://example.org/onto/prop/google_apihub_plugin_instance_update">
    <rdfs:label>update</rdfs:label>
    <rdfs:domain rdf:resource="http://example.org/onto/class/google_apihub_plugin_instance"/>
    <rdfs:range rdf:resource="http://www.w3.org/2001/XMLSchema#string"/>
  </owl:DatatypeProperty>
</rdf:RDF>
