<?xml version="1.0" encoding="UTF-8"?>
<rdf:RDF
  xmlns:rdf="http://www.w3.org/1999/02/22-rdf-syntax-ns#"
  xmlns:rdfs="http://www.w3.org/2000/01/rdf-schema#"
  xmlns:owl="http://www.w3.org/2002/07/owl#"
  xmlns:xsd="http://www.w3.org/2001/XMLSchema#"
  xml:base="http://example.org/onto/">
  <owl:Class rdf:about="http://example.org/onto/class/google_bigquery_reservation">
    <rdfs:label>google_bigquery_reservation</rdfs:label>
    <rdfs:comment>#
#     ***     AUTO GENERATED CODE    ***    Type: MMv1     ***
#
# ----------------------------------------------------------------------------
#
#     This code is generated by Magic Modules using the following:
#
#     Configuration: https:#github.com/GoogleCloudPlatform/magic-modules/tree/main/mmv1/products/bigqueryreservation/Reservation.yaml
#     Template:      https:#github.com/GoogleCloudPlatform/magic-modules/tree/main/mmv1/templates/terraform/resource.html.markdown.tmpl
#
#     DO NOT EDIT this file directly. Any changes made to this file will be
#     overwritten during the next generation cycle.
#
# ----------------------------------------------------------------------------
subcategory: "BigQuery Reservation"
description: |-
  A reservation is a mechanism used to guarantee BigQuery slots to users.
---</rdfs:comment>
  </owl:Class>
  <owl:DatatypeProperty rdf:about="http://example.org/onto/prop/google_bigquery_reservation_concurrency">
    <rdfs:label>concurrency</rdfs:label>
    <rdfs:comment>Maximum number of queries that are allowed to run concurrently in this reservation. This is a soft limit due to asynchronous nature of the system and various optimizations for small queries. Default value is 0 which means that concurrency will be automatically set based on the reservation size.</rdfs:comment>
    <rdfs:domain rdf:resource="http://example.org/onto/class/google_bigquery_reservation"/>
    <rdfs:range rdf:resource="http://www.w3.org/2001/XMLSchema#string"/>
  </owl:DatatypeProperty>
  <owl:DatatypeProperty rdf:about="http://example.org/onto/prop/google_bigquery_reservation_edition">
    <rdfs:label>edition</rdfs:label>
    <rdfs:comment>The edition type. Valid values are STANDARD, ENTERPRISE, ENTERPRISE_PLUS</rdfs:comment>
    <rdfs:domain rdf:resource="http://example.org/onto/class/google_bigquery_reservation"/>
    <rdfs:range rdf:resource="http://www.w3.org/2001/XMLSchema#string"/>
  </owl:DatatypeProperty>
  <owl:DatatypeProperty rdf:about="http://example.org/onto/prop/google_bigquery_reservation_id">
    <rdfs:label>id</rdfs:label>
    <rdfs:domain rdf:resource="http://example.org/onto/class/google_bigquery_reservation"/>
    <rdfs:range rdf:resource="http://www.w3.org/2001/XMLSchema#string"/>
  </owl:DatatypeProperty>
  <owl:DatatypeProperty rdf:about="http://example.org/onto/prop/google_bigquery_reservation_ignore_idle_slots">
    <rdfs:label>ignore_idle_slots</rdfs:label>
    <rdfs:comment>If false, any query using this reservation will use idle slots from other reservations within
the same admin project. If true, a query using this reservation will execute with the slot
capacity specified above at most.</rdfs:comment>
    <rdfs:domain rdf:resource="http://example.org/onto/class/google_bigquery_reservation"/>
    <rdfs:range rdf:resource="http://www.w3.org/2001/XMLSchema#string"/>
  </owl:DatatypeProperty>
  <owl:DatatypeProperty rdf:about="http://example.org/onto/prop/google_bigquery_reservation_location">
    <rdfs:label>location</rdfs:label>
    <rdfs:comment>The geographic location where the transfer config should reside.
Examples: US, EU, asia-northeast1. The default value is US.</rdfs:comment>
    <rdfs:domain rdf:resource="http://example.org/onto/class/google_bigquery_reservation"/>
    <rdfs:range rdf:resource="http://www.w3.org/2001/XMLSchema#string"/>
  </owl:DatatypeProperty>
  <owl:DatatypeProperty rdf:about="http://example.org/onto/prop/google_bigquery_reservation_name">
    <rdfs:label>name</rdfs:label>
    <rdfs:comment>The name of the reservation. This field must only contain alphanumeric characters or dash.</rdfs:comment>
    <rdfs:domain rdf:resource="http://example.org/onto/class/google_bigquery_reservation"/>
    <rdfs:range rdf:resource="http://www.w3.org/2001/XMLSchema#string"/>
  </owl:DatatypeProperty>
  <owl:DatatypeProperty rdf:about="http://example.org/onto/prop/google_bigquery_reservation_original_primary_location">
    <rdfs:label>original_primary_location</rdfs:label>
    <rdfs:comment>The location where the reservation was originally created. This is set only during the
failover reservation's creation. All billing charges for the failover reservation will be
applied to this location.</rdfs:comment>
    <rdfs:domain rdf:resource="http://example.org/onto/class/google_bigquery_reservation"/>
    <rdfs:range rdf:resource="http://www.w3.org/2001/XMLSchema#string"/>
  </owl:DatatypeProperty>
  <owl:DatatypeProperty rdf:about="http://example.org/onto/prop/google_bigquery_reservation_primary_location">
    <rdfs:label>primary_location</rdfs:label>
    <rdfs:comment>The current location of the reservation's primary replica. This field is only set for
reservations using the managed disaster recovery feature.</rdfs:comment>
    <rdfs:domain rdf:resource="http://example.org/onto/class/google_bigquery_reservation"/>
    <rdfs:range rdf:resource="http://www.w3.org/2001/XMLSchema#string"/>
  </owl:DatatypeProperty>
  <owl:DatatypeProperty rdf:about="http://example.org/onto/prop/google_bigquery_reservation_project">
    <rdfs:label>project</rdfs:label>
    <rdfs:domain rdf:resource="http://example.org/onto/class/google_bigquery_reservation"/>
    <rdfs:range rdf:resource="http://www.w3.org/2001/XMLSchema#string"/>
  </owl:DatatypeProperty>
  <owl:DatatypeProperty rdf:about="http://example.org/onto/prop/google_bigquery_reservation_replication_status">
    <rdfs:label>replication_status</rdfs:label>
    <rdfs:comment>The Disaster Recovery(DR) replication status of the reservation. This is only available for
the primary replicas of DR/failover reservations and provides information about the both the
staleness of the secondary and the last error encountered while trying to replicate changes
from the primary to the secondary. If this field is blank, it means that the reservation is
either not a DR reservation or the reservation is a DR secondary or that any replication
operations on the reservation have succeeded.</rdfs:comment>
    <rdfs:domain rdf:resource="http://example.org/onto/class/google_bigquery_reservation"/>
    <rdfs:range rdf:resource="http://www.w3.org/2001/XMLSchema#string"/>
  </owl:DatatypeProperty>
  <owl:DatatypeProperty rdf:about="http://example.org/onto/prop/google_bigquery_reservation_secondary_location">
    <rdfs:label>secondary_location</rdfs:label>
    <rdfs:comment>The current location of the reservation's secondary replica. This field is only set for
reservations using the managed disaster recovery feature. Users can set this in create
reservation calls to create a failover reservation or in update reservation calls to convert
a non-failover reservation to a failover reservation(or vice versa).</rdfs:comment>
    <rdfs:domain rdf:resource="http://example.org/onto/class/google_bigquery_reservation"/>
    <rdfs:range rdf:resource="http://www.w3.org/2001/XMLSchema#string"/>
  </owl:DatatypeProperty>
  <owl:DatatypeProperty rdf:about="http://example.org/onto/prop/google_bigquery_reservation_slot_capacity">
    <rdfs:label>slot_capacity</rdfs:label>
    <rdfs:comment>Minimum slots available to this reservation. A slot is a unit of computational power in BigQuery, and serves as the
unit of parallelism. Queries using this reservation might use more slots during runtime if ignoreIdleSlots is set to false.</rdfs:comment>
    <rdfs:domain rdf:resource="http://example.org/onto/class/google_bigquery_reservation"/>
    <rdfs:range rdf:resource="http://www.w3.org/2001/XMLSchema#string"/>
  </owl:DatatypeProperty>
  <owl:DatatypeProperty rdf:about="http://example.org/onto/prop/google_bigquery_reservation_current_slots">
    <rdfs:label>current_slots</rdfs:label>
    <rdfs:comment>The slot capacity added to this reservation when autoscale happens. Will be between [0, max_slots].</rdfs:comment>
    <rdfs:domain rdf:resource="http://example.org/onto/class/google_bigquery_reservation"/>
    <rdfs:range rdf:resource="http://www.w3.org/2001/XMLSchema#string"/>
  </owl:DatatypeProperty>
  <owl:DatatypeProperty rdf:about="http://example.org/onto/prop/google_bigquery_reservation_max_slots">
    <rdfs:label>max_slots</rdfs:label>
    <rdfs:comment>Number of slots to be scaled when needed.</rdfs:comment>
    <rdfs:domain rdf:resource="http://example.org/onto/class/google_bigquery_reservation"/>
    <rdfs:range rdf:resource="http://www.w3.org/2001/XMLSchema#string"/>
  </owl:DatatypeProperty>
  <owl:DatatypeProperty rdf:about="http://example.org/onto/prop/google_bigquery_reservation_create">
    <rdfs:label>create</rdfs:label>
    <rdfs:domain rdf:resource="http://example.org/onto/class/google_bigquery_reservation"/>
    <rdfs:range rdf:resource="http://www.w3.org/2001/XMLSchema#string"/>
  </owl:DatatypeProperty>
  <owl:DatatypeProperty rdf:about="http://example.org/onto/prop/google_bigquery_reservation_delete">
    <rdfs:label>delete</rdfs:label>
    <rdfs:domain rdf:resource="http://example.org/onto/class/google_bigquery_reservation"/>
    <rdfs:range rdf:resource="http://www.w3.org/2001/XMLSchema#string"/>
  </owl:DatatypeProperty>
  <owl:DatatypeProperty rdf:about="http://example.org/onto/prop/google_bigquery_reservation_update">
    <rdfs:label>update</rdfs:label>
    <rdfs:domain rdf:resource="http://example.org/onto/class/google_bigquery_reservation"/>
    <rdfs:range rdf:resource="http://www.w3.org/2001/XMLSchema#string"/>
  </owl:DatatypeProperty>
</rdf:RDF>
