<?xml version="1.0" encoding="UTF-8"?>
<rdf:RDF
  xmlns:rdf="http://www.w3.org/1999/02/22-rdf-syntax-ns#"
  xmlns:rdfs="http://www.w3.org/2000/01/rdf-schema#"
  xmlns:owl="http://www.w3.org/2002/07/owl#"
  xmlns:xsd="http://www.w3.org/2001/XMLSchema#"
  xml:base="http://example.org/onto/">
  <owl:Class rdf:about="http://example.org/onto/class/google_compute_interconnect_attachment">
    <rdfs:label>google_compute_interconnect_attachment</rdfs:label>
    <rdfs:comment>#
#     ***     AUTO GENERATED CODE    ***    Type: MMv1     ***
#
# ----------------------------------------------------------------------------
#
#     This code is generated by Magic Modules using the following:
#
#     Configuration: https:#github.com/GoogleCloudPlatform/magic-modules/tree/main/mmv1/products/compute/InterconnectAttachment.yaml
#     Template:      https:#github.com/GoogleCloudPlatform/magic-modules/tree/main/mmv1/templates/terraform/resource.html.markdown.tmpl
#
#     DO NOT EDIT this file directly. Any changes made to this file will be
#     overwritten during the next generation cycle.
#
# ----------------------------------------------------------------------------
subcategory: "Compute Engine"
description: |-
  Represents an InterconnectAttachment (VLAN attachment) resource.
---</rdfs:comment>
  </owl:Class>
  <owl:DatatypeProperty rdf:about="http://example.org/onto/prop/google_compute_interconnect_attachment_admin_enabled">
    <rdfs:label>admin_enabled</rdfs:label>
    <rdfs:comment>Whether the VLAN attachment is enabled or disabled.  When using
PARTNER type this will Pre-Activate the interconnect attachment</rdfs:comment>
    <rdfs:domain rdf:resource="http://example.org/onto/class/google_compute_interconnect_attachment"/>
    <rdfs:range rdf:resource="http://www.w3.org/2001/XMLSchema#string"/>
  </owl:DatatypeProperty>
  <owl:DatatypeProperty rdf:about="http://example.org/onto/prop/google_compute_interconnect_attachment_attachment_group">
    <rdfs:label>attachment_group</rdfs:label>
    <rdfs:comment>URL of the AttachmentGroup that includes this Attachment.</rdfs:comment>
    <rdfs:domain rdf:resource="http://example.org/onto/class/google_compute_interconnect_attachment"/>
    <rdfs:range rdf:resource="http://www.w3.org/2001/XMLSchema#string"/>
  </owl:DatatypeProperty>
  <owl:DatatypeProperty rdf:about="http://example.org/onto/prop/google_compute_interconnect_attachment_bandwidth">
    <rdfs:label>bandwidth</rdfs:label>
    <rdfs:comment>Provisioned bandwidth capacity for the interconnect attachment.
For attachments of type DEDICATED, the user can set the bandwidth.
For attachments of type PARTNER, the Google Partner that is operating the interconnect must set the bandwidth.
Output only for PARTNER type, mutable for PARTNER_PROVIDER and DEDICATED,
Defaults to BPS_10G Possible values: ["BPS_50M", "BPS_100M", "BPS_200M", "BPS_300M", "BPS_400M", "BPS_500M", "BPS_1G", "BPS_2G", "BPS_5G", "BPS_10G", "BPS_20G", "BPS_50G", "BPS_100G"]</rdfs:comment>
    <rdfs:domain rdf:resource="http://example.org/onto/class/google_compute_interconnect_attachment"/>
    <rdfs:range rdf:resource="http://www.w3.org/2001/XMLSchema#string"/>
  </owl:DatatypeProperty>
  <owl:DatatypeProperty rdf:about="http://example.org/onto/prop/google_compute_interconnect_attachment_candidate_subnets">
    <rdfs:label>candidate_subnets</rdfs:label>
    <rdfs:comment>Up to 16 candidate prefixes that can be used to restrict the allocation
of cloudRouterIpAddress and customerRouterIpAddress for this attachment.
All prefixes must be within link-local address space (169.254.0.0/16)
and must be /29 or shorter (/28, /27, etc). Google will attempt to select
an unused /29 from the supplied candidate prefix(es). The request will
fail if all possible /29s are in use on Google's edge. If not supplied,
Google will randomly select an unused /29 from all of link-local space.</rdfs:comment>
    <rdfs:domain rdf:resource="http://example.org/onto/class/google_compute_interconnect_attachment"/>
    <rdfs:range rdf:resource="http://www.w3.org/2001/XMLSchema#string"/>
  </owl:DatatypeProperty>
  <owl:DatatypeProperty rdf:about="http://example.org/onto/prop/google_compute_interconnect_attachment_cloud_router_ip_address">
    <rdfs:label>cloud_router_ip_address</rdfs:label>
    <rdfs:comment>IPv4 address + prefix length to be configured on Cloud Router
Interface for this interconnect attachment.</rdfs:comment>
    <rdfs:domain rdf:resource="http://example.org/onto/class/google_compute_interconnect_attachment"/>
    <rdfs:range rdf:resource="http://www.w3.org/2001/XMLSchema#string"/>
  </owl:DatatypeProperty>
  <owl:DatatypeProperty rdf:about="http://example.org/onto/prop/google_compute_interconnect_attachment_cloud_router_ipv6_address">
    <rdfs:label>cloud_router_ipv6_address</rdfs:label>
    <rdfs:comment>IPv6 address + prefix length to be configured on Cloud Router
Interface for this interconnect attachment.</rdfs:comment>
    <rdfs:domain rdf:resource="http://example.org/onto/class/google_compute_interconnect_attachment"/>
    <rdfs:range rdf:resource="http://www.w3.org/2001/XMLSchema#string"/>
  </owl:DatatypeProperty>
  <owl:DatatypeProperty rdf:about="http://example.org/onto/prop/google_compute_interconnect_attachment_creation_timestamp">
    <rdfs:label>creation_timestamp</rdfs:label>
    <rdfs:comment>Creation timestamp in RFC3339 text format.</rdfs:comment>
    <rdfs:domain rdf:resource="http://example.org/onto/class/google_compute_interconnect_attachment"/>
    <rdfs:range rdf:resource="http://www.w3.org/2001/XMLSchema#string"/>
  </owl:DatatypeProperty>
  <owl:DatatypeProperty rdf:about="http://example.org/onto/prop/google_compute_interconnect_attachment_customer_router_ip_address">
    <rdfs:label>customer_router_ip_address</rdfs:label>
    <rdfs:comment>IPv4 address + prefix length to be configured on the customer
router subinterface for this interconnect attachment.</rdfs:comment>
    <rdfs:domain rdf:resource="http://example.org/onto/class/google_compute_interconnect_attachment"/>
    <rdfs:range rdf:resource="http://www.w3.org/2001/XMLSchema#string"/>
  </owl:DatatypeProperty>
  <owl:DatatypeProperty rdf:about="http://example.org/onto/prop/google_compute_interconnect_attachment_customer_router_ipv6_address">
    <rdfs:label>customer_router_ipv6_address</rdfs:label>
    <rdfs:comment>IPv6 address + prefix length to be configured on the customer
router subinterface for this interconnect attachment.</rdfs:comment>
    <rdfs:domain rdf:resource="http://example.org/onto/class/google_compute_interconnect_attachment"/>
    <rdfs:range rdf:resource="http://www.w3.org/2001/XMLSchema#string"/>
  </owl:DatatypeProperty>
  <owl:DatatypeProperty rdf:about="http://example.org/onto/prop/google_compute_interconnect_attachment_description">
    <rdfs:label>description</rdfs:label>
    <rdfs:comment>An optional description of this resource.</rdfs:comment>
    <rdfs:domain rdf:resource="http://example.org/onto/class/google_compute_interconnect_attachment"/>
    <rdfs:range rdf:resource="http://www.w3.org/2001/XMLSchema#string"/>
  </owl:DatatypeProperty>
  <owl:DatatypeProperty rdf:about="http://example.org/onto/prop/google_compute_interconnect_attachment_edge_availability_domain">
    <rdfs:label>edge_availability_domain</rdfs:label>
    <rdfs:comment>Desired availability domain for the attachment. Only available for type
PARTNER, at creation time. For improved reliability, customers should
configure a pair of attachments with one per availability domain. The
selected availability domain will be provided to the Partner via the
pairing key so that the provisioned circuit will lie in the specified
domain. If not specified, the value will default to AVAILABILITY_DOMAIN_ANY.</rdfs:comment>
    <rdfs:domain rdf:resource="http://example.org/onto/class/google_compute_interconnect_attachment"/>
    <rdfs:range rdf:resource="http://www.w3.org/2001/XMLSchema#string"/>
  </owl:DatatypeProperty>
  <owl:DatatypeProperty rdf:about="http://example.org/onto/prop/google_compute_interconnect_attachment_effective_labels">
    <rdfs:label>effective_labels</rdfs:label>
    <rdfs:comment>All of labels (key/value pairs) present on the resource in GCP, including the labels configured through Terraform, other clients and services.</rdfs:comment>
    <rdfs:domain rdf:resource="http://example.org/onto/class/google_compute_interconnect_attachment"/>
    <rdfs:range rdf:resource="http://www.w3.org/2001/XMLSchema#string"/>
  </owl:DatatypeProperty>
  <owl:DatatypeProperty rdf:about="http://example.org/onto/prop/google_compute_interconnect_attachment_encryption">
    <rdfs:label>encryption</rdfs:label>
    <rdfs:comment>Indicates the user-supplied encryption option of this interconnect
attachment. Can only be specified at attachment creation for PARTNER or
DEDICATED attachments.
* NONE - This is the default value, which means that the VLAN attachment
carries unencrypted traffic. VMs are able to send traffic to, or receive
traffic from, such a VLAN attachment.
* IPSEC - The VLAN attachment carries only encrypted traffic that is
encrypted by an IPsec device, such as an HA VPN gateway or third-party
IPsec VPN. VMs cannot directly send traffic to, or receive traffic from,
such a VLAN attachment. To use HA VPN over Cloud Interconnect, the VLAN
attachment must be created with this option. Default value: "NONE" Possible values: ["NONE", "IPSEC"]</rdfs:comment>
    <rdfs:domain rdf:resource="http://example.org/onto/class/google_compute_interconnect_attachment"/>
    <rdfs:range rdf:resource="http://www.w3.org/2001/XMLSchema#string"/>
  </owl:DatatypeProperty>
  <owl:DatatypeProperty rdf:about="http://example.org/onto/prop/google_compute_interconnect_attachment_google_reference_id">
    <rdfs:label>google_reference_id</rdfs:label>
    <rdfs:comment>Google reference ID, to be used when raising support tickets with
Google or otherwise to debug backend connectivity issues.</rdfs:comment>
    <rdfs:domain rdf:resource="http://example.org/onto/class/google_compute_interconnect_attachment"/>
    <rdfs:range rdf:resource="http://www.w3.org/2001/XMLSchema#string"/>
  </owl:DatatypeProperty>
  <owl:DatatypeProperty rdf:about="http://example.org/onto/prop/google_compute_interconnect_attachment_id">
    <rdfs:label>id</rdfs:label>
    <rdfs:domain rdf:resource="http://example.org/onto/class/google_compute_interconnect_attachment"/>
    <rdfs:range rdf:resource="http://www.w3.org/2001/XMLSchema#string"/>
  </owl:DatatypeProperty>
  <owl:DatatypeProperty rdf:about="http://example.org/onto/prop/google_compute_interconnect_attachment_interconnect">
    <rdfs:label>interconnect</rdfs:label>
    <rdfs:comment>URL of the underlying Interconnect object that this attachment's
traffic will traverse through. Required if type is DEDICATED, must not
be set if type is PARTNER.</rdfs:comment>
    <rdfs:domain rdf:resource="http://example.org/onto/class/google_compute_interconnect_attachment"/>
    <rdfs:range rdf:resource="http://www.w3.org/2001/XMLSchema#string"/>
  </owl:DatatypeProperty>
  <owl:DatatypeProperty rdf:about="http://example.org/onto/prop/google_compute_interconnect_attachment_ipsec_internal_addresses">
    <rdfs:label>ipsec_internal_addresses</rdfs:label>
    <rdfs:comment>URL of addresses that have been reserved for the interconnect attachment,
Used only for interconnect attachment that has the encryption option as
IPSEC.
The addresses must be RFC 1918 IP address ranges. When creating HA VPN
gateway over the interconnect attachment, if the attachment is configured
to use an RFC 1918 IP address, then the VPN gateway's IP address will be
allocated from the IP address range specified here.
For example, if the HA VPN gateway's interface 0 is paired to this
interconnect attachment, then an RFC 1918 IP address for the VPN gateway
interface 0 will be allocated from the IP address specified for this
interconnect attachment.
If this field is not specified for interconnect attachment that has
encryption option as IPSEC, later on when creating HA VPN gateway on this
interconnect attachment, the HA VPN gateway's IP address will be
allocated from regional external IP address pool.</rdfs:comment>
    <rdfs:domain rdf:resource="http://example.org/onto/class/google_compute_interconnect_attachment"/>
    <rdfs:range rdf:resource="http://www.w3.org/2001/XMLSchema#string"/>
  </owl:DatatypeProperty>
  <owl:DatatypeProperty rdf:about="http://example.org/onto/prop/google_compute_interconnect_attachment_label_fingerprint">
    <rdfs:label>label_fingerprint</rdfs:label>
    <rdfs:comment>A fingerprint for the labels being applied to this Interconnect, which is essentially a hash
of the labels set used for optimistic locking. The fingerprint is initially generated by
Compute Engine and changes after every request to modify or update labels.
You must always provide an up-to-date fingerprint hash in order to update or change labels,
otherwise the request will fail with error 412 conditionNotMet.</rdfs:comment>
    <rdfs:domain rdf:resource="http://example.org/onto/class/google_compute_interconnect_attachment"/>
    <rdfs:range rdf:resource="http://www.w3.org/2001/XMLSchema#string"/>
  </owl:DatatypeProperty>
  <owl:DatatypeProperty rdf:about="http://example.org/onto/prop/google_compute_interconnect_attachment_labels">
    <rdfs:label>labels</rdfs:label>
    <rdfs:comment>Labels for this resource. These can only be added or modified by the setLabels
method. Each label key/value pair must comply with RFC1035. Label values may be empty.


**Note**: This field is non-authoritative, and will only manage the labels present in your configuration.
Please refer to the field 'effective_labels' for all of the labels present on the resource.</rdfs:comment>
    <rdfs:domain rdf:resource="http://example.org/onto/class/google_compute_interconnect_attachment"/>
    <rdfs:range rdf:resource="http://www.w3.org/2001/XMLSchema#string"/>
  </owl:DatatypeProperty>
  <owl:DatatypeProperty rdf:about="http://example.org/onto/prop/google_compute_interconnect_attachment_mtu">
    <rdfs:label>mtu</rdfs:label>
    <rdfs:comment>Maximum Transmission Unit (MTU), in bytes, of packets passing through this interconnect attachment.
Valid values are 1440, 1460, 1500, and 8896. If not specified, the value will default to 1440.</rdfs:comment>
    <rdfs:domain rdf:resource="http://example.org/onto/class/google_compute_interconnect_attachment"/>
    <rdfs:range rdf:resource="http://www.w3.org/2001/XMLSchema#string"/>
  </owl:DatatypeProperty>
  <owl:DatatypeProperty rdf:about="http://example.org/onto/prop/google_compute_interconnect_attachment_name">
    <rdfs:label>name</rdfs:label>
    <rdfs:comment>Name of the resource. Provided by the client when the resource is created. The
name must be 1-63 characters long, and comply with RFC1035. Specifically, the
name must be 1-63 characters long and match the regular expression
'[a-z]([-a-z0-9]*[a-z0-9])?' which means the first character must be a
lowercase letter, and all following characters must be a dash, lowercase
letter, or digit, except the last character, which cannot be a dash.</rdfs:comment>
    <rdfs:domain rdf:resource="http://example.org/onto/class/google_compute_interconnect_attachment"/>
    <rdfs:range rdf:resource="http://www.w3.org/2001/XMLSchema#string"/>
  </owl:DatatypeProperty>
  <owl:DatatypeProperty rdf:about="http://example.org/onto/prop/google_compute_interconnect_attachment_pairing_key">
    <rdfs:label>pairing_key</rdfs:label>
    <rdfs:comment>[Output only for type PARTNER. Not present for DEDICATED]. The opaque
identifier of an PARTNER attachment used to initiate provisioning with
a selected partner. Of the form "XXXXX/region/domain"</rdfs:comment>
    <rdfs:domain rdf:resource="http://example.org/onto/class/google_compute_interconnect_attachment"/>
    <rdfs:range rdf:resource="http://www.w3.org/2001/XMLSchema#string"/>
  </owl:DatatypeProperty>
  <owl:DatatypeProperty rdf:about="http://example.org/onto/prop/google_compute_interconnect_attachment_partner_asn">
    <rdfs:label>partner_asn</rdfs:label>
    <rdfs:comment>[Output only for type PARTNER. Not present for DEDICATED]. Optional
BGP ASN for the router that should be supplied by a layer 3 Partner if
they configured BGP on behalf of the customer.</rdfs:comment>
    <rdfs:domain rdf:resource="http://example.org/onto/class/google_compute_interconnect_attachment"/>
    <rdfs:range rdf:resource="http://www.w3.org/2001/XMLSchema#string"/>
  </owl:DatatypeProperty>
  <owl:DatatypeProperty rdf:about="http://example.org/onto/prop/google_compute_interconnect_attachment_private_interconnect_info">
    <rdfs:label>private_interconnect_info</rdfs:label>
    <rdfs:comment>Information specific to an InterconnectAttachment. This property
is populated if the interconnect that this is attached to is of type DEDICATED.</rdfs:comment>
    <rdfs:domain rdf:resource="http://example.org/onto/class/google_compute_interconnect_attachment"/>
    <rdfs:range rdf:resource="http://www.w3.org/2001/XMLSchema#string"/>
  </owl:DatatypeProperty>
  <owl:DatatypeProperty rdf:about="http://example.org/onto/prop/google_compute_interconnect_attachment_project">
    <rdfs:label>project</rdfs:label>
    <rdfs:domain rdf:resource="http://example.org/onto/class/google_compute_interconnect_attachment"/>
    <rdfs:range rdf:resource="http://www.w3.org/2001/XMLSchema#string"/>
  </owl:DatatypeProperty>
  <owl:DatatypeProperty rdf:about="http://example.org/onto/prop/google_compute_interconnect_attachment_region">
    <rdfs:label>region</rdfs:label>
    <rdfs:comment>Region where the regional interconnect attachment resides.</rdfs:comment>
    <rdfs:domain rdf:resource="http://example.org/onto/class/google_compute_interconnect_attachment"/>
    <rdfs:range rdf:resource="http://www.w3.org/2001/XMLSchema#string"/>
  </owl:DatatypeProperty>
  <owl:DatatypeProperty rdf:about="http://example.org/onto/prop/google_compute_interconnect_attachment_router">
    <rdfs:label>router</rdfs:label>
    <rdfs:comment>URL of the cloud router to be used for dynamic routing. This router must be in
the same region as this InterconnectAttachment. The InterconnectAttachment will
automatically connect the Interconnect to the network & region within which the
Cloud Router is configured.</rdfs:comment>
    <rdfs:domain rdf:resource="http://example.org/onto/class/google_compute_interconnect_attachment"/>
    <rdfs:range rdf:resource="http://www.w3.org/2001/XMLSchema#string"/>
  </owl:DatatypeProperty>
  <owl:DatatypeProperty rdf:about="http://example.org/onto/prop/google_compute_interconnect_attachment_self_link">
    <rdfs:label>self_link</rdfs:label>
    <rdfs:domain rdf:resource="http://example.org/onto/class/google_compute_interconnect_attachment"/>
    <rdfs:range rdf:resource="http://www.w3.org/2001/XMLSchema#string"/>
  </owl:DatatypeProperty>
  <owl:DatatypeProperty rdf:about="http://example.org/onto/prop/google_compute_interconnect_attachment_stack_type">
    <rdfs:label>stack_type</rdfs:label>
    <rdfs:comment>The stack type for this interconnect attachment to identify whether the IPv6
feature is enabled or not. If not specified, IPV4_ONLY will be used.
This field can be both set at interconnect attachments creation and update
interconnect attachment operations. Possible values: ["IPV4_IPV6", "IPV4_ONLY"]</rdfs:comment>
    <rdfs:domain rdf:resource="http://example.org/onto/class/google_compute_interconnect_attachment"/>
    <rdfs:range rdf:resource="http://www.w3.org/2001/XMLSchema#string"/>
  </owl:DatatypeProperty>
  <owl:DatatypeProperty rdf:about="http://example.org/onto/prop/google_compute_interconnect_attachment_state">
    <rdfs:label>state</rdfs:label>
    <rdfs:comment>[Output Only] The current state of this attachment's functionality.</rdfs:comment>
    <rdfs:domain rdf:resource="http://example.org/onto/class/google_compute_interconnect_attachment"/>
    <rdfs:range rdf:resource="http://www.w3.org/2001/XMLSchema#string"/>
  </owl:DatatypeProperty>
  <owl:DatatypeProperty rdf:about="http://example.org/onto/prop/google_compute_interconnect_attachment_subnet_length">
    <rdfs:label>subnet_length</rdfs:label>
    <rdfs:comment>Length of the IPv4 subnet mask. Allowed values: 29 (default), 30. The default value is 29,
except for Cross-Cloud Interconnect connections that use an InterconnectRemoteLocation with a
constraints.subnetLengthRange.min equal to 30. For example, connections that use an Azure
remote location fall into this category. In these cases, the default value is 30, and
requesting 29 returns an error. Where both 29 and 30 are allowed, 29 is preferred, because it
gives Google Cloud Support more debugging visibility.</rdfs:comment>
    <rdfs:domain rdf:resource="http://example.org/onto/class/google_compute_interconnect_attachment"/>
    <rdfs:range rdf:resource="http://www.w3.org/2001/XMLSchema#string"/>
  </owl:DatatypeProperty>
  <owl:DatatypeProperty rdf:about="http://example.org/onto/prop/google_compute_interconnect_attachment_terraform_labels">
    <rdfs:label>terraform_labels</rdfs:label>
    <rdfs:comment>The combination of labels configured directly on the resource
 and default labels configured on the provider.</rdfs:comment>
    <rdfs:domain rdf:resource="http://example.org/onto/class/google_compute_interconnect_attachment"/>
    <rdfs:range rdf:resource="http://www.w3.org/2001/XMLSchema#string"/>
  </owl:DatatypeProperty>
  <owl:DatatypeProperty rdf:about="http://example.org/onto/prop/google_compute_interconnect_attachment_type">
    <rdfs:label>type</rdfs:label>
    <rdfs:comment>The type of InterconnectAttachment you wish to create. Defaults to
DEDICATED. Possible values: ["DEDICATED", "PARTNER", "PARTNER_PROVIDER"]</rdfs:comment>
    <rdfs:domain rdf:resource="http://example.org/onto/class/google_compute_interconnect_attachment"/>
    <rdfs:range rdf:resource="http://www.w3.org/2001/XMLSchema#string"/>
  </owl:DatatypeProperty>
  <owl:DatatypeProperty rdf:about="http://example.org/onto/prop/google_compute_interconnect_attachment_vlan_tag8021q">
    <rdfs:label>vlan_tag8021q</rdfs:label>
    <rdfs:comment>The IEEE 802.1Q VLAN tag for this attachment, in the range 2-4094. When
using PARTNER type this will be managed upstream.</rdfs:comment>
    <rdfs:domain rdf:resource="http://example.org/onto/class/google_compute_interconnect_attachment"/>
    <rdfs:range rdf:resource="http://www.w3.org/2001/XMLSchema#string"/>
  </owl:DatatypeProperty>
  <owl:DatatypeProperty rdf:about="http://example.org/onto/prop/google_compute_interconnect_attachment_create">
    <rdfs:label>create</rdfs:label>
    <rdfs:domain rdf:resource="http://example.org/onto/class/google_compute_interconnect_attachment"/>
    <rdfs:range rdf:resource="http://www.w3.org/2001/XMLSchema#string"/>
  </owl:DatatypeProperty>
  <owl:DatatypeProperty rdf:about="http://example.org/onto/prop/google_compute_interconnect_attachment_delete">
    <rdfs:label>delete</rdfs:label>
    <rdfs:domain rdf:resource="http://example.org/onto/class/google_compute_interconnect_attachment"/>
    <rdfs:range rdf:resource="http://www.w3.org/2001/XMLSchema#string"/>
  </owl:DatatypeProperty>
  <owl:DatatypeProperty rdf:about="http://example.org/onto/prop/google_compute_interconnect_attachment_update">
    <rdfs:label>update</rdfs:label>
    <rdfs:domain rdf:resource="http://example.org/onto/class/google_compute_interconnect_attachment"/>
    <rdfs:range rdf:resource="http://www.w3.org/2001/XMLSchema#string"/>
  </owl:DatatypeProperty>
</rdf:RDF>
