<?xml version="1.0" encoding="UTF-8"?>
<rdf:RDF
  xmlns:rdf="http://www.w3.org/1999/02/22-rdf-syntax-ns#"
  xmlns:rdfs="http://www.w3.org/2000/01/rdf-schema#"
  xmlns:owl="http://www.w3.org/2002/07/owl#"
  xmlns:xsd="http://www.w3.org/2001/XMLSchema#"
  xml:base="http://example.org/onto/">
  <owl:Class rdf:about="http://example.org/onto/class/google_network_connectivity_service_connection_policy">
    <rdfs:label>google_network_connectivity_service_connection_policy</rdfs:label>
    <rdfs:comment>#
#     ***     AUTO GENERATED CODE    ***    Type: MMv1     ***
#
# ----------------------------------------------------------------------------
#
#     This code is generated by Magic Modules using the following:
#
#     Configuration: https:#github.com/GoogleCloudPlatform/magic-modules/tree/main/mmv1/products/networkconnectivityv1/ServiceConnectionPolicy.yaml
#     Template:      https:#github.com/GoogleCloudPlatform/magic-modules/tree/main/mmv1/templates/terraform/resource.html.markdown.tmpl
#
#     DO NOT EDIT this file directly. Any changes made to this file will be
#     overwritten during the next generation cycle.
#
# ----------------------------------------------------------------------------
subcategory: "Network Connectivity"
description: |-
  Manage Service Connection Policies.
---</rdfs:comment>
  </owl:Class>
  <owl:DatatypeProperty rdf:about="http://example.org/onto/prop/google_network_connectivity_service_connection_policy_create_time">
    <rdfs:label>create_time</rdfs:label>
    <rdfs:comment>The timestamp when the resource was created.</rdfs:comment>
    <rdfs:domain rdf:resource="http://example.org/onto/class/google_network_connectivity_service_connection_policy"/>
    <rdfs:range rdf:resource="http://www.w3.org/2001/XMLSchema#string"/>
  </owl:DatatypeProperty>
  <owl:DatatypeProperty rdf:about="http://example.org/onto/prop/google_network_connectivity_service_connection_policy_description">
    <rdfs:label>description</rdfs:label>
    <rdfs:comment>Free-text description of the resource.</rdfs:comment>
    <rdfs:domain rdf:resource="http://example.org/onto/class/google_network_connectivity_service_connection_policy"/>
    <rdfs:range rdf:resource="http://www.w3.org/2001/XMLSchema#string"/>
  </owl:DatatypeProperty>
  <owl:DatatypeProperty rdf:about="http://example.org/onto/prop/google_network_connectivity_service_connection_policy_effective_labels">
    <rdfs:label>effective_labels</rdfs:label>
    <rdfs:comment>All of labels (key/value pairs) present on the resource in GCP, including the labels configured through Terraform, other clients and services.</rdfs:comment>
    <rdfs:domain rdf:resource="http://example.org/onto/class/google_network_connectivity_service_connection_policy"/>
    <rdfs:range rdf:resource="http://www.w3.org/2001/XMLSchema#string"/>
  </owl:DatatypeProperty>
  <owl:DatatypeProperty rdf:about="http://example.org/onto/prop/google_network_connectivity_service_connection_policy_etag">
    <rdfs:label>etag</rdfs:label>
    <rdfs:comment>The etag is computed by the server, and may be sent on update and delete requests to ensure the client has an up-to-date value before proceeding.</rdfs:comment>
    <rdfs:domain rdf:resource="http://example.org/onto/class/google_network_connectivity_service_connection_policy"/>
    <rdfs:range rdf:resource="http://www.w3.org/2001/XMLSchema#string"/>
  </owl:DatatypeProperty>
  <owl:DatatypeProperty rdf:about="http://example.org/onto/prop/google_network_connectivity_service_connection_policy_id">
    <rdfs:label>id</rdfs:label>
    <rdfs:domain rdf:resource="http://example.org/onto/class/google_network_connectivity_service_connection_policy"/>
    <rdfs:range rdf:resource="http://www.w3.org/2001/XMLSchema#string"/>
  </owl:DatatypeProperty>
  <owl:DatatypeProperty rdf:about="http://example.org/onto/prop/google_network_connectivity_service_connection_policy_infrastructure">
    <rdfs:label>infrastructure</rdfs:label>
    <rdfs:comment>The type of underlying resources used to create the connection.</rdfs:comment>
    <rdfs:domain rdf:resource="http://example.org/onto/class/google_network_connectivity_service_connection_policy"/>
    <rdfs:range rdf:resource="http://www.w3.org/2001/XMLSchema#string"/>
  </owl:DatatypeProperty>
  <owl:DatatypeProperty rdf:about="http://example.org/onto/prop/google_network_connectivity_service_connection_policy_labels">
    <rdfs:label>labels</rdfs:label>
    <rdfs:comment>User-defined labels.


**Note**: This field is non-authoritative, and will only manage the labels present in your configuration.
Please refer to the field 'effective_labels' for all of the labels present on the resource.</rdfs:comment>
    <rdfs:domain rdf:resource="http://example.org/onto/class/google_network_connectivity_service_connection_policy"/>
    <rdfs:range rdf:resource="http://www.w3.org/2001/XMLSchema#string"/>
  </owl:DatatypeProperty>
  <owl:DatatypeProperty rdf:about="http://example.org/onto/prop/google_network_connectivity_service_connection_policy_location">
    <rdfs:label>location</rdfs:label>
    <rdfs:comment>The location of the ServiceConnectionPolicy.</rdfs:comment>
    <rdfs:domain rdf:resource="http://example.org/onto/class/google_network_connectivity_service_connection_policy"/>
    <rdfs:range rdf:resource="http://www.w3.org/2001/XMLSchema#string"/>
  </owl:DatatypeProperty>
  <owl:DatatypeProperty rdf:about="http://example.org/onto/prop/google_network_connectivity_service_connection_policy_name">
    <rdfs:label>name</rdfs:label>
    <rdfs:comment>The name of a ServiceConnectionPolicy. Format: projects/{project}/locations/{location}/serviceConnectionPolicies/{service_connection_policy} See: https://google.aip.dev/122#fields-representing-resource-names</rdfs:comment>
    <rdfs:domain rdf:resource="http://example.org/onto/class/google_network_connectivity_service_connection_policy"/>
    <rdfs:range rdf:resource="http://www.w3.org/2001/XMLSchema#string"/>
  </owl:DatatypeProperty>
  <owl:DatatypeProperty rdf:about="http://example.org/onto/prop/google_network_connectivity_service_connection_policy_network">
    <rdfs:label>network</rdfs:label>
    <rdfs:comment>The resource path of the consumer network. Example: - projects/{projectNumOrId}/global/networks/{resourceId}.</rdfs:comment>
    <rdfs:domain rdf:resource="http://example.org/onto/class/google_network_connectivity_service_connection_policy"/>
    <rdfs:range rdf:resource="http://www.w3.org/2001/XMLSchema#string"/>
  </owl:DatatypeProperty>
  <owl:DatatypeProperty rdf:about="http://example.org/onto/prop/google_network_connectivity_service_connection_policy_project">
    <rdfs:label>project</rdfs:label>
    <rdfs:domain rdf:resource="http://example.org/onto/class/google_network_connectivity_service_connection_policy"/>
    <rdfs:range rdf:resource="http://www.w3.org/2001/XMLSchema#string"/>
  </owl:DatatypeProperty>
  <owl:DatatypeProperty rdf:about="http://example.org/onto/prop/google_network_connectivity_service_connection_policy_psc_connections">
    <rdfs:label>psc_connections</rdfs:label>
    <rdfs:comment>Information about each Private Service Connect connection.</rdfs:comment>
    <rdfs:domain rdf:resource="http://example.org/onto/class/google_network_connectivity_service_connection_policy"/>
    <rdfs:range rdf:resource="http://www.w3.org/2001/XMLSchema#string"/>
  </owl:DatatypeProperty>
  <owl:DatatypeProperty rdf:about="http://example.org/onto/prop/google_network_connectivity_service_connection_policy_service_class">
    <rdfs:label>service_class</rdfs:label>
    <rdfs:comment>The service class identifier for which this ServiceConnectionPolicy is for. The service class identifier is a unique, symbolic representation of a ServiceClass.
It is provided by the Service Producer. Google services have a prefix of gcp. For example, gcp-cloud-sql. 3rd party services do not. For example, test-service-a3dfcx.</rdfs:comment>
    <rdfs:domain rdf:resource="http://example.org/onto/class/google_network_connectivity_service_connection_policy"/>
    <rdfs:range rdf:resource="http://www.w3.org/2001/XMLSchema#string"/>
  </owl:DatatypeProperty>
  <owl:DatatypeProperty rdf:about="http://example.org/onto/prop/google_network_connectivity_service_connection_policy_terraform_labels">
    <rdfs:label>terraform_labels</rdfs:label>
    <rdfs:comment>The combination of labels configured directly on the resource
 and default labels configured on the provider.</rdfs:comment>
    <rdfs:domain rdf:resource="http://example.org/onto/class/google_network_connectivity_service_connection_policy"/>
    <rdfs:range rdf:resource="http://www.w3.org/2001/XMLSchema#string"/>
  </owl:DatatypeProperty>
  <owl:DatatypeProperty rdf:about="http://example.org/onto/prop/google_network_connectivity_service_connection_policy_update_time">
    <rdfs:label>update_time</rdfs:label>
    <rdfs:comment>The timestamp when the resource was updated.</rdfs:comment>
    <rdfs:domain rdf:resource="http://example.org/onto/class/google_network_connectivity_service_connection_policy"/>
    <rdfs:range rdf:resource="http://www.w3.org/2001/XMLSchema#string"/>
  </owl:DatatypeProperty>
  <owl:DatatypeProperty rdf:about="http://example.org/onto/prop/google_network_connectivity_service_connection_policy_allowed_google_producers_resource_hierarchy_level">
    <rdfs:label>allowed_google_producers_resource_hierarchy_level</rdfs:label>
    <rdfs:comment>List of Projects, Folders, or Organizations from where the Producer instance can be within. For example,
a network administrator can provide both 'organizations/foo' and 'projects/bar' as
allowed_google_producers_resource_hierarchy_levels. This allowlists this network to connect with any Producer
instance within the 'foo' organization or the 'bar' project. By default,
allowedGoogleProducersResourceHierarchyLevel is empty. The format for each
allowedGoogleProducersResourceHierarchyLevel is / where is one of 'projects', 'folders', or 'organizations'
and is either the ID or the number of the resource type. Format for each
allowedGoogleProducersResourceHierarchyLevel value: 'projects/' or 'folders/' or 'organizations/' Eg.
[projects/my-project-id, projects/567, folders/891, organizations/123]</rdfs:comment>
    <rdfs:domain rdf:resource="http://example.org/onto/class/google_network_connectivity_service_connection_policy"/>
    <rdfs:range rdf:resource="http://www.w3.org/2001/XMLSchema#string"/>
  </owl:DatatypeProperty>
  <owl:DatatypeProperty rdf:about="http://example.org/onto/prop/google_network_connectivity_service_connection_policy_limit">
    <rdfs:label>limit</rdfs:label>
    <rdfs:comment>Max number of PSC connections for this policy.</rdfs:comment>
    <rdfs:domain rdf:resource="http://example.org/onto/class/google_network_connectivity_service_connection_policy"/>
    <rdfs:range rdf:resource="http://www.w3.org/2001/XMLSchema#string"/>
  </owl:DatatypeProperty>
  <owl:DatatypeProperty rdf:about="http://example.org/onto/prop/google_network_connectivity_service_connection_policy_producer_instance_location">
    <rdfs:label>producer_instance_location</rdfs:label>
    <rdfs:comment>ProducerInstanceLocation is used to specify which authorization mechanism to use to determine which projects
the Producer instance can be within. Possible values: ["PRODUCER_INSTANCE_LOCATION_UNSPECIFIED", "CUSTOM_RESOURCE_HIERARCHY_LEVELS"]</rdfs:comment>
    <rdfs:domain rdf:resource="http://example.org/onto/class/google_network_connectivity_service_connection_policy"/>
    <rdfs:range rdf:resource="http://www.w3.org/2001/XMLSchema#string"/>
  </owl:DatatypeProperty>
  <owl:DatatypeProperty rdf:about="http://example.org/onto/prop/google_network_connectivity_service_connection_policy_subnetworks">
    <rdfs:label>subnetworks</rdfs:label>
    <rdfs:comment>IDs of the subnetworks or fully qualified identifiers for the subnetworks</rdfs:comment>
    <rdfs:domain rdf:resource="http://example.org/onto/class/google_network_connectivity_service_connection_policy"/>
    <rdfs:range rdf:resource="http://www.w3.org/2001/XMLSchema#string"/>
  </owl:DatatypeProperty>
  <owl:DatatypeProperty rdf:about="http://example.org/onto/prop/google_network_connectivity_service_connection_policy_create">
    <rdfs:label>create</rdfs:label>
    <rdfs:domain rdf:resource="http://example.org/onto/class/google_network_connectivity_service_connection_policy"/>
    <rdfs:range rdf:resource="http://www.w3.org/2001/XMLSchema#string"/>
  </owl:DatatypeProperty>
  <owl:DatatypeProperty rdf:about="http://example.org/onto/prop/google_network_connectivity_service_connection_policy_delete">
    <rdfs:label>delete</rdfs:label>
    <rdfs:domain rdf:resource="http://example.org/onto/class/google_network_connectivity_service_connection_policy"/>
    <rdfs:range rdf:resource="http://www.w3.org/2001/XMLSchema#string"/>
  </owl:DatatypeProperty>
  <owl:DatatypeProperty rdf:about="http://example.org/onto/prop/google_network_connectivity_service_connection_policy_update">
    <rdfs:label>update</rdfs:label>
    <rdfs:domain rdf:resource="http://example.org/onto/class/google_network_connectivity_service_connection_policy"/>
    <rdfs:range rdf:resource="http://www.w3.org/2001/XMLSchema#string"/>
  </owl:DatatypeProperty>
</rdf:RDF>
