<?xml version="1.0" encoding="UTF-8"?>
<rdf:RDF
  xmlns:rdf="http://www.w3.org/1999/02/22-rdf-syntax-ns#"
  xmlns:rdfs="http://www.w3.org/2000/01/rdf-schema#"
  xmlns:owl="http://www.w3.org/2002/07/owl#"
  xmlns:xsd="http://www.w3.org/2001/XMLSchema#"
  xml:base="http://example.org/onto/">
  <owl:Class rdf:about="http://example.org/onto/class/google_oracle_database_cloud_exadata_infrastructure">
    <rdfs:label>google_oracle_database_cloud_exadata_infrastructure</rdfs:label>
    <rdfs:comment>#
#     ***     AUTO GENERATED CODE    ***    Type: MMv1     ***
#
# ----------------------------------------------------------------------------
#
#     This code is generated by Magic Modules using the following:
#
#     Configuration: https:#github.com/GoogleCloudPlatform/magic-modules/tree/main/mmv1/products/oracledatabase/CloudExadataInfrastructure.yaml
#     Template:      https:#github.com/GoogleCloudPlatform/magic-modules/tree/main/mmv1/templates/terraform/resource.html.markdown.tmpl
#
#     DO NOT EDIT this file directly. Any changes made to this file will be
#     overwritten during the next generation cycle.
#
# ----------------------------------------------------------------------------
subcategory: "Oracle Database"
description: |-
  A CloudExadataInfrastructure resource.
---</rdfs:comment>
  </owl:Class>
  <owl:DatatypeProperty rdf:about="http://example.org/onto/prop/google_oracle_database_cloud_exadata_infrastructure_cloud_exadata_infrastructure_id">
    <rdfs:label>cloud_exadata_infrastructure_id</rdfs:label>
    <rdfs:comment>The ID of the Exadata Infrastructure to create. This value is restricted
to (^[a-z]([a-z0-9-]{0,61}[a-z0-9])?$) and must be a maximum of 63
characters in length. The value must start with a letter and end with
a letter or a number.</rdfs:comment>
    <rdfs:domain rdf:resource="http://example.org/onto/class/google_oracle_database_cloud_exadata_infrastructure"/>
    <rdfs:range rdf:resource="http://www.w3.org/2001/XMLSchema#string"/>
  </owl:DatatypeProperty>
  <owl:DatatypeProperty rdf:about="http://example.org/onto/prop/google_oracle_database_cloud_exadata_infrastructure_create_time">
    <rdfs:label>create_time</rdfs:label>
    <rdfs:comment>The date and time that the Exadata Infrastructure was created.</rdfs:comment>
    <rdfs:domain rdf:resource="http://example.org/onto/class/google_oracle_database_cloud_exadata_infrastructure"/>
    <rdfs:range rdf:resource="http://www.w3.org/2001/XMLSchema#string"/>
  </owl:DatatypeProperty>
  <owl:DatatypeProperty rdf:about="http://example.org/onto/prop/google_oracle_database_cloud_exadata_infrastructure_deletion_protection">
    <rdfs:label>deletion_protection</rdfs:label>
    <rdfs:comment>Whether or not to allow Terraform to destroy the instance. Unless this field is set to false in Terraform state, a terraform destroy or terraform apply that would delete the instance will fail.</rdfs:comment>
    <rdfs:domain rdf:resource="http://example.org/onto/class/google_oracle_database_cloud_exadata_infrastructure"/>
    <rdfs:range rdf:resource="http://www.w3.org/2001/XMLSchema#string"/>
  </owl:DatatypeProperty>
  <owl:DatatypeProperty rdf:about="http://example.org/onto/prop/google_oracle_database_cloud_exadata_infrastructure_display_name">
    <rdfs:label>display_name</rdfs:label>
    <rdfs:comment>User friendly name for this resource.</rdfs:comment>
    <rdfs:domain rdf:resource="http://example.org/onto/class/google_oracle_database_cloud_exadata_infrastructure"/>
    <rdfs:range rdf:resource="http://www.w3.org/2001/XMLSchema#string"/>
  </owl:DatatypeProperty>
  <owl:DatatypeProperty rdf:about="http://example.org/onto/prop/google_oracle_database_cloud_exadata_infrastructure_effective_labels">
    <rdfs:label>effective_labels</rdfs:label>
    <rdfs:comment>All of labels (key/value pairs) present on the resource in GCP, including the labels configured through Terraform, other clients and services.</rdfs:comment>
    <rdfs:domain rdf:resource="http://example.org/onto/class/google_oracle_database_cloud_exadata_infrastructure"/>
    <rdfs:range rdf:resource="http://www.w3.org/2001/XMLSchema#string"/>
  </owl:DatatypeProperty>
  <owl:DatatypeProperty rdf:about="http://example.org/onto/prop/google_oracle_database_cloud_exadata_infrastructure_entitlement_id">
    <rdfs:label>entitlement_id</rdfs:label>
    <rdfs:comment>Entitlement ID of the private offer against which this infrastructure
resource is provisioned.</rdfs:comment>
    <rdfs:domain rdf:resource="http://example.org/onto/class/google_oracle_database_cloud_exadata_infrastructure"/>
    <rdfs:range rdf:resource="http://www.w3.org/2001/XMLSchema#string"/>
  </owl:DatatypeProperty>
  <owl:DatatypeProperty rdf:about="http://example.org/onto/prop/google_oracle_database_cloud_exadata_infrastructure_gcp_oracle_zone">
    <rdfs:label>gcp_oracle_zone</rdfs:label>
    <rdfs:comment>GCP location where Oracle Exadata is hosted.</rdfs:comment>
    <rdfs:domain rdf:resource="http://example.org/onto/class/google_oracle_database_cloud_exadata_infrastructure"/>
    <rdfs:range rdf:resource="http://www.w3.org/2001/XMLSchema#string"/>
  </owl:DatatypeProperty>
  <owl:DatatypeProperty rdf:about="http://example.org/onto/prop/google_oracle_database_cloud_exadata_infrastructure_id">
    <rdfs:label>id</rdfs:label>
    <rdfs:domain rdf:resource="http://example.org/onto/class/google_oracle_database_cloud_exadata_infrastructure"/>
    <rdfs:range rdf:resource="http://www.w3.org/2001/XMLSchema#string"/>
  </owl:DatatypeProperty>
  <owl:DatatypeProperty rdf:about="http://example.org/onto/prop/google_oracle_database_cloud_exadata_infrastructure_labels">
    <rdfs:label>labels</rdfs:label>
    <rdfs:comment>Labels or tags associated with the resource. 

**Note**: This field is non-authoritative, and will only manage the labels present in your configuration.
Please refer to the field 'effective_labels' for all of the labels present on the resource.</rdfs:comment>
    <rdfs:domain rdf:resource="http://example.org/onto/class/google_oracle_database_cloud_exadata_infrastructure"/>
    <rdfs:range rdf:resource="http://www.w3.org/2001/XMLSchema#string"/>
  </owl:DatatypeProperty>
  <owl:DatatypeProperty rdf:about="http://example.org/onto/prop/google_oracle_database_cloud_exadata_infrastructure_location">
    <rdfs:label>location</rdfs:label>
    <rdfs:comment>Resource ID segment making up resource 'name'. See documentation for resource type 'oracledatabase.googleapis.com/DbServer'.</rdfs:comment>
    <rdfs:domain rdf:resource="http://example.org/onto/class/google_oracle_database_cloud_exadata_infrastructure"/>
    <rdfs:range rdf:resource="http://www.w3.org/2001/XMLSchema#string"/>
  </owl:DatatypeProperty>
  <owl:DatatypeProperty rdf:about="http://example.org/onto/prop/google_oracle_database_cloud_exadata_infrastructure_name">
    <rdfs:label>name</rdfs:label>
    <rdfs:comment>Identifier. The name of the Exadata Infrastructure resource with the following format:
projects/{project}/locations/{region}/cloudExadataInfrastructures/{cloud_exadata_infrastructure}</rdfs:comment>
    <rdfs:domain rdf:resource="http://example.org/onto/class/google_oracle_database_cloud_exadata_infrastructure"/>
    <rdfs:range rdf:resource="http://www.w3.org/2001/XMLSchema#string"/>
  </owl:DatatypeProperty>
  <owl:DatatypeProperty rdf:about="http://example.org/onto/prop/google_oracle_database_cloud_exadata_infrastructure_project">
    <rdfs:label>project</rdfs:label>
    <rdfs:domain rdf:resource="http://example.org/onto/class/google_oracle_database_cloud_exadata_infrastructure"/>
    <rdfs:range rdf:resource="http://www.w3.org/2001/XMLSchema#string"/>
  </owl:DatatypeProperty>
  <owl:DatatypeProperty rdf:about="http://example.org/onto/prop/google_oracle_database_cloud_exadata_infrastructure_terraform_labels">
    <rdfs:label>terraform_labels</rdfs:label>
    <rdfs:comment>The combination of labels configured directly on the resource
 and default labels configured on the provider.</rdfs:comment>
    <rdfs:domain rdf:resource="http://example.org/onto/class/google_oracle_database_cloud_exadata_infrastructure"/>
    <rdfs:range rdf:resource="http://www.w3.org/2001/XMLSchema#string"/>
  </owl:DatatypeProperty>
  <owl:DatatypeProperty rdf:about="http://example.org/onto/prop/google_oracle_database_cloud_exadata_infrastructure_activated_storage_count">
    <rdfs:label>activated_storage_count</rdfs:label>
    <rdfs:comment>The requested number of additional storage servers activated for the
Exadata Infrastructure.</rdfs:comment>
    <rdfs:domain rdf:resource="http://example.org/onto/class/google_oracle_database_cloud_exadata_infrastructure"/>
    <rdfs:range rdf:resource="http://www.w3.org/2001/XMLSchema#string"/>
  </owl:DatatypeProperty>
  <owl:DatatypeProperty rdf:about="http://example.org/onto/prop/google_oracle_database_cloud_exadata_infrastructure_additional_storage_count">
    <rdfs:label>additional_storage_count</rdfs:label>
    <rdfs:comment>The requested number of additional storage servers for the Exadata
Infrastructure.</rdfs:comment>
    <rdfs:domain rdf:resource="http://example.org/onto/class/google_oracle_database_cloud_exadata_infrastructure"/>
    <rdfs:range rdf:resource="http://www.w3.org/2001/XMLSchema#string"/>
  </owl:DatatypeProperty>
  <owl:DatatypeProperty rdf:about="http://example.org/onto/prop/google_oracle_database_cloud_exadata_infrastructure_available_storage_size_gb">
    <rdfs:label>available_storage_size_gb</rdfs:label>
    <rdfs:comment>The available storage can be allocated to the Exadata Infrastructure
resource, in gigabytes (GB).</rdfs:comment>
    <rdfs:domain rdf:resource="http://example.org/onto/class/google_oracle_database_cloud_exadata_infrastructure"/>
    <rdfs:range rdf:resource="http://www.w3.org/2001/XMLSchema#string"/>
  </owl:DatatypeProperty>
  <owl:DatatypeProperty rdf:about="http://example.org/onto/prop/google_oracle_database_cloud_exadata_infrastructure_compute_count">
    <rdfs:label>compute_count</rdfs:label>
    <rdfs:comment>The number of compute servers for the Exadata Infrastructure.</rdfs:comment>
    <rdfs:domain rdf:resource="http://example.org/onto/class/google_oracle_database_cloud_exadata_infrastructure"/>
    <rdfs:range rdf:resource="http://www.w3.org/2001/XMLSchema#string"/>
  </owl:DatatypeProperty>
  <owl:DatatypeProperty rdf:about="http://example.org/onto/prop/google_oracle_database_cloud_exadata_infrastructure_cpu_count">
    <rdfs:label>cpu_count</rdfs:label>
    <rdfs:comment>The number of enabled CPU cores.</rdfs:comment>
    <rdfs:domain rdf:resource="http://example.org/onto/class/google_oracle_database_cloud_exadata_infrastructure"/>
    <rdfs:range rdf:resource="http://www.w3.org/2001/XMLSchema#string"/>
  </owl:DatatypeProperty>
  <owl:DatatypeProperty rdf:about="http://example.org/onto/prop/google_oracle_database_cloud_exadata_infrastructure_data_storage_size_tb">
    <rdfs:label>data_storage_size_tb</rdfs:label>
    <rdfs:comment>Size, in terabytes, of the DATA disk group.</rdfs:comment>
    <rdfs:domain rdf:resource="http://example.org/onto/class/google_oracle_database_cloud_exadata_infrastructure"/>
    <rdfs:range rdf:resource="http://www.w3.org/2001/XMLSchema#string"/>
  </owl:DatatypeProperty>
  <owl:DatatypeProperty rdf:about="http://example.org/onto/prop/google_oracle_database_cloud_exadata_infrastructure_db_node_storage_size_gb">
    <rdfs:label>db_node_storage_size_gb</rdfs:label>
    <rdfs:comment>The local node storage allocated in GBs.</rdfs:comment>
    <rdfs:domain rdf:resource="http://example.org/onto/class/google_oracle_database_cloud_exadata_infrastructure"/>
    <rdfs:range rdf:resource="http://www.w3.org/2001/XMLSchema#string"/>
  </owl:DatatypeProperty>
  <owl:DatatypeProperty rdf:about="http://example.org/onto/prop/google_oracle_database_cloud_exadata_infrastructure_db_server_version">
    <rdfs:label>db_server_version</rdfs:label>
    <rdfs:comment>The software version of the database servers (dom0) in the Exadata
Infrastructure.</rdfs:comment>
    <rdfs:domain rdf:resource="http://example.org/onto/class/google_oracle_database_cloud_exadata_infrastructure"/>
    <rdfs:range rdf:resource="http://www.w3.org/2001/XMLSchema#string"/>
  </owl:DatatypeProperty>
  <owl:DatatypeProperty rdf:about="http://example.org/onto/prop/google_oracle_database_cloud_exadata_infrastructure_max_cpu_count">
    <rdfs:label>max_cpu_count</rdfs:label>
    <rdfs:comment>The total number of CPU cores available.</rdfs:comment>
    <rdfs:domain rdf:resource="http://example.org/onto/class/google_oracle_database_cloud_exadata_infrastructure"/>
    <rdfs:range rdf:resource="http://www.w3.org/2001/XMLSchema#string"/>
  </owl:DatatypeProperty>
  <owl:DatatypeProperty rdf:about="http://example.org/onto/prop/google_oracle_database_cloud_exadata_infrastructure_max_data_storage_tb">
    <rdfs:label>max_data_storage_tb</rdfs:label>
    <rdfs:comment>The total available DATA disk group size.</rdfs:comment>
    <rdfs:domain rdf:resource="http://example.org/onto/class/google_oracle_database_cloud_exadata_infrastructure"/>
    <rdfs:range rdf:resource="http://www.w3.org/2001/XMLSchema#string"/>
  </owl:DatatypeProperty>
  <owl:DatatypeProperty rdf:about="http://example.org/onto/prop/google_oracle_database_cloud_exadata_infrastructure_max_db_node_storage_size_gb">
    <rdfs:label>max_db_node_storage_size_gb</rdfs:label>
    <rdfs:comment>The total local node storage available in GBs.</rdfs:comment>
    <rdfs:domain rdf:resource="http://example.org/onto/class/google_oracle_database_cloud_exadata_infrastructure"/>
    <rdfs:range rdf:resource="http://www.w3.org/2001/XMLSchema#string"/>
  </owl:DatatypeProperty>
  <owl:DatatypeProperty rdf:about="http://example.org/onto/prop/google_oracle_database_cloud_exadata_infrastructure_max_memory_gb">
    <rdfs:label>max_memory_gb</rdfs:label>
    <rdfs:comment>The total memory available in GBs.</rdfs:comment>
    <rdfs:domain rdf:resource="http://example.org/onto/class/google_oracle_database_cloud_exadata_infrastructure"/>
    <rdfs:range rdf:resource="http://www.w3.org/2001/XMLSchema#string"/>
  </owl:DatatypeProperty>
  <owl:DatatypeProperty rdf:about="http://example.org/onto/prop/google_oracle_database_cloud_exadata_infrastructure_memory_size_gb">
    <rdfs:label>memory_size_gb</rdfs:label>
    <rdfs:comment>The memory allocated in GBs.</rdfs:comment>
    <rdfs:domain rdf:resource="http://example.org/onto/class/google_oracle_database_cloud_exadata_infrastructure"/>
    <rdfs:range rdf:resource="http://www.w3.org/2001/XMLSchema#string"/>
  </owl:DatatypeProperty>
  <owl:DatatypeProperty rdf:about="http://example.org/onto/prop/google_oracle_database_cloud_exadata_infrastructure_monthly_db_server_version">
    <rdfs:label>monthly_db_server_version</rdfs:label>
    <rdfs:comment>The monthly software version of the database servers (dom0)
in the Exadata Infrastructure. Example: 20.1.15</rdfs:comment>
    <rdfs:domain rdf:resource="http://example.org/onto/class/google_oracle_database_cloud_exadata_infrastructure"/>
    <rdfs:range rdf:resource="http://www.w3.org/2001/XMLSchema#string"/>
  </owl:DatatypeProperty>
  <owl:DatatypeProperty rdf:about="http://example.org/onto/prop/google_oracle_database_cloud_exadata_infrastructure_monthly_storage_server_version">
    <rdfs:label>monthly_storage_server_version</rdfs:label>
    <rdfs:comment>The monthly software version of the storage servers (cells)
in the Exadata Infrastructure. Example: 20.1.15</rdfs:comment>
    <rdfs:domain rdf:resource="http://example.org/onto/class/google_oracle_database_cloud_exadata_infrastructure"/>
    <rdfs:range rdf:resource="http://www.w3.org/2001/XMLSchema#string"/>
  </owl:DatatypeProperty>
  <owl:DatatypeProperty rdf:about="http://example.org/onto/prop/google_oracle_database_cloud_exadata_infrastructure_next_maintenance_run_id">
    <rdfs:label>next_maintenance_run_id</rdfs:label>
    <rdfs:comment>The OCID of the next maintenance run.</rdfs:comment>
    <rdfs:domain rdf:resource="http://example.org/onto/class/google_oracle_database_cloud_exadata_infrastructure"/>
    <rdfs:range rdf:resource="http://www.w3.org/2001/XMLSchema#string"/>
  </owl:DatatypeProperty>
  <owl:DatatypeProperty rdf:about="http://example.org/onto/prop/google_oracle_database_cloud_exadata_infrastructure_next_maintenance_run_time">
    <rdfs:label>next_maintenance_run_time</rdfs:label>
    <rdfs:comment>The time when the next maintenance run will occur.</rdfs:comment>
    <rdfs:domain rdf:resource="http://example.org/onto/class/google_oracle_database_cloud_exadata_infrastructure"/>
    <rdfs:range rdf:resource="http://www.w3.org/2001/XMLSchema#string"/>
  </owl:DatatypeProperty>
  <owl:DatatypeProperty rdf:about="http://example.org/onto/prop/google_oracle_database_cloud_exadata_infrastructure_next_security_maintenance_run_time">
    <rdfs:label>next_security_maintenance_run_time</rdfs:label>
    <rdfs:comment>The time when the next security maintenance run will occur.</rdfs:comment>
    <rdfs:domain rdf:resource="http://example.org/onto/class/google_oracle_database_cloud_exadata_infrastructure"/>
    <rdfs:range rdf:resource="http://www.w3.org/2001/XMLSchema#string"/>
  </owl:DatatypeProperty>
  <owl:DatatypeProperty rdf:about="http://example.org/onto/prop/google_oracle_database_cloud_exadata_infrastructure_oci_url">
    <rdfs:label>oci_url</rdfs:label>
    <rdfs:comment>Deep link to the OCI console to view this resource.</rdfs:comment>
    <rdfs:domain rdf:resource="http://example.org/onto/class/google_oracle_database_cloud_exadata_infrastructure"/>
    <rdfs:range rdf:resource="http://www.w3.org/2001/XMLSchema#string"/>
  </owl:DatatypeProperty>
  <owl:DatatypeProperty rdf:about="http://example.org/onto/prop/google_oracle_database_cloud_exadata_infrastructure_ocid">
    <rdfs:label>ocid</rdfs:label>
    <rdfs:comment>OCID of created infra.
https://docs.oracle.com/en-us/iaas/Content/General/Concepts/identifiers.htm#Oracle</rdfs:comment>
    <rdfs:domain rdf:resource="http://example.org/onto/class/google_oracle_database_cloud_exadata_infrastructure"/>
    <rdfs:range rdf:resource="http://www.w3.org/2001/XMLSchema#string"/>
  </owl:DatatypeProperty>
  <owl:DatatypeProperty rdf:about="http://example.org/onto/prop/google_oracle_database_cloud_exadata_infrastructure_shape">
    <rdfs:label>shape</rdfs:label>
    <rdfs:comment>The shape of the Exadata Infrastructure. The shape determines the
amount of CPU, storage, and memory resources allocated to the instance.</rdfs:comment>
    <rdfs:domain rdf:resource="http://example.org/onto/class/google_oracle_database_cloud_exadata_infrastructure"/>
    <rdfs:range rdf:resource="http://www.w3.org/2001/XMLSchema#string"/>
  </owl:DatatypeProperty>
  <owl:DatatypeProperty rdf:about="http://example.org/onto/prop/google_oracle_database_cloud_exadata_infrastructure_state">
    <rdfs:label>state</rdfs:label>
    <rdfs:comment>The current lifecycle state of the Exadata Infrastructure. 
 Possible values:
 STATE_UNSPECIFIED
PROVISIONING
AVAILABLE
UPDATING
TERMINATING
TERMINATED
FAILED
MAINTENANCE_IN_PROGRESS</rdfs:comment>
    <rdfs:domain rdf:resource="http://example.org/onto/class/google_oracle_database_cloud_exadata_infrastructure"/>
    <rdfs:range rdf:resource="http://www.w3.org/2001/XMLSchema#string"/>
  </owl:DatatypeProperty>
  <owl:DatatypeProperty rdf:about="http://example.org/onto/prop/google_oracle_database_cloud_exadata_infrastructure_storage_count">
    <rdfs:label>storage_count</rdfs:label>
    <rdfs:comment>The number of Cloud Exadata storage servers for the Exadata Infrastructure.</rdfs:comment>
    <rdfs:domain rdf:resource="http://example.org/onto/class/google_oracle_database_cloud_exadata_infrastructure"/>
    <rdfs:range rdf:resource="http://www.w3.org/2001/XMLSchema#string"/>
  </owl:DatatypeProperty>
  <owl:DatatypeProperty rdf:about="http://example.org/onto/prop/google_oracle_database_cloud_exadata_infrastructure_storage_server_version">
    <rdfs:label>storage_server_version</rdfs:label>
    <rdfs:comment>The software version of the storage servers (cells) in the Exadata
Infrastructure.</rdfs:comment>
    <rdfs:domain rdf:resource="http://example.org/onto/class/google_oracle_database_cloud_exadata_infrastructure"/>
    <rdfs:range rdf:resource="http://www.w3.org/2001/XMLSchema#string"/>
  </owl:DatatypeProperty>
  <owl:DatatypeProperty rdf:about="http://example.org/onto/prop/google_oracle_database_cloud_exadata_infrastructure_total_storage_size_gb">
    <rdfs:label>total_storage_size_gb</rdfs:label>
    <rdfs:comment>The total storage allocated to the Exadata Infrastructure
resource, in gigabytes (GB).</rdfs:comment>
    <rdfs:domain rdf:resource="http://example.org/onto/class/google_oracle_database_cloud_exadata_infrastructure"/>
    <rdfs:range rdf:resource="http://www.w3.org/2001/XMLSchema#string"/>
  </owl:DatatypeProperty>
  <owl:DatatypeProperty rdf:about="http://example.org/onto/prop/google_oracle_database_cloud_exadata_infrastructure_email">
    <rdfs:label>email</rdfs:label>
    <rdfs:comment>The email address used by Oracle to send notifications regarding databases
and infrastructure.</rdfs:comment>
    <rdfs:domain rdf:resource="http://example.org/onto/class/google_oracle_database_cloud_exadata_infrastructure"/>
    <rdfs:range rdf:resource="http://www.w3.org/2001/XMLSchema#string"/>
  </owl:DatatypeProperty>
  <owl:DatatypeProperty rdf:about="http://example.org/onto/prop/google_oracle_database_cloud_exadata_infrastructure_custom_action_timeout_mins">
    <rdfs:label>custom_action_timeout_mins</rdfs:label>
    <rdfs:comment>Determines the amount of time the system will wait before the start of each
database server patching operation. Custom action timeout is in minutes and
valid value is between 15 to 120 (inclusive).</rdfs:comment>
    <rdfs:domain rdf:resource="http://example.org/onto/class/google_oracle_database_cloud_exadata_infrastructure"/>
    <rdfs:range rdf:resource="http://www.w3.org/2001/XMLSchema#string"/>
  </owl:DatatypeProperty>
  <owl:DatatypeProperty rdf:about="http://example.org/onto/prop/google_oracle_database_cloud_exadata_infrastructure_days_of_week">
    <rdfs:label>days_of_week</rdfs:label>
    <rdfs:comment>Days during the week when maintenance should be performed.</rdfs:comment>
    <rdfs:domain rdf:resource="http://example.org/onto/class/google_oracle_database_cloud_exadata_infrastructure"/>
    <rdfs:range rdf:resource="http://www.w3.org/2001/XMLSchema#string"/>
  </owl:DatatypeProperty>
  <owl:DatatypeProperty rdf:about="http://example.org/onto/prop/google_oracle_database_cloud_exadata_infrastructure_hours_of_day">
    <rdfs:label>hours_of_day</rdfs:label>
    <rdfs:comment>The window of hours during the day when maintenance should be performed.
The window is a 4 hour slot. Valid values are:
  0 - represents time slot 0:00 - 3:59 UTC
  4 - represents time slot 4:00 - 7:59 UTC
  8 - represents time slot 8:00 - 11:59 UTC
  12 - represents time slot 12:00 - 15:59 UTC
  16 - represents time slot 16:00 - 19:59 UTC
  20 - represents time slot 20:00 - 23:59 UTC</rdfs:comment>
    <rdfs:domain rdf:resource="http://example.org/onto/class/google_oracle_database_cloud_exadata_infrastructure"/>
    <rdfs:range rdf:resource="http://www.w3.org/2001/XMLSchema#string"/>
  </owl:DatatypeProperty>
  <owl:DatatypeProperty rdf:about="http://example.org/onto/prop/google_oracle_database_cloud_exadata_infrastructure_is_custom_action_timeout_enabled">
    <rdfs:label>is_custom_action_timeout_enabled</rdfs:label>
    <rdfs:comment>If true, enables the configuration of a custom action timeout (waiting
period) between database server patching operations.</rdfs:comment>
    <rdfs:domain rdf:resource="http://example.org/onto/class/google_oracle_database_cloud_exadata_infrastructure"/>
    <rdfs:range rdf:resource="http://www.w3.org/2001/XMLSchema#string"/>
  </owl:DatatypeProperty>
  <owl:DatatypeProperty rdf:about="http://example.org/onto/prop/google_oracle_database_cloud_exadata_infrastructure_lead_time_week">
    <rdfs:label>lead_time_week</rdfs:label>
    <rdfs:comment>Lead time window allows user to set a lead time to prepare for a down time.
The lead time is in weeks and valid value is between 1 to 4.</rdfs:comment>
    <rdfs:domain rdf:resource="http://example.org/onto/class/google_oracle_database_cloud_exadata_infrastructure"/>
    <rdfs:range rdf:resource="http://www.w3.org/2001/XMLSchema#string"/>
  </owl:DatatypeProperty>
  <owl:DatatypeProperty rdf:about="http://example.org/onto/prop/google_oracle_database_cloud_exadata_infrastructure_months">
    <rdfs:label>months</rdfs:label>
    <rdfs:comment>Months during the year when maintenance should be performed.</rdfs:comment>
    <rdfs:domain rdf:resource="http://example.org/onto/class/google_oracle_database_cloud_exadata_infrastructure"/>
    <rdfs:range rdf:resource="http://www.w3.org/2001/XMLSchema#string"/>
  </owl:DatatypeProperty>
  <owl:DatatypeProperty rdf:about="http://example.org/onto/prop/google_oracle_database_cloud_exadata_infrastructure_patching_mode">
    <rdfs:label>patching_mode</rdfs:label>
    <rdfs:comment>Cloud CloudExadataInfrastructure node patching method, either "ROLLING"
 or "NONROLLING". Default value is ROLLING. 
 Possible values:
 PATCHING_MODE_UNSPECIFIED
ROLLING
NON_ROLLING</rdfs:comment>
    <rdfs:domain rdf:resource="http://example.org/onto/class/google_oracle_database_cloud_exadata_infrastructure"/>
    <rdfs:range rdf:resource="http://www.w3.org/2001/XMLSchema#string"/>
  </owl:DatatypeProperty>
  <owl:DatatypeProperty rdf:about="http://example.org/onto/prop/google_oracle_database_cloud_exadata_infrastructure_preference">
    <rdfs:label>preference</rdfs:label>
    <rdfs:comment>The maintenance window scheduling preference. 
 Possible values:
 MAINTENANCE_WINDOW_PREFERENCE_UNSPECIFIED
CUSTOM_PREFERENCE
NO_PREFERENCE</rdfs:comment>
    <rdfs:domain rdf:resource="http://example.org/onto/class/google_oracle_database_cloud_exadata_infrastructure"/>
    <rdfs:range rdf:resource="http://www.w3.org/2001/XMLSchema#string"/>
  </owl:DatatypeProperty>
  <owl:DatatypeProperty rdf:about="http://example.org/onto/prop/google_oracle_database_cloud_exadata_infrastructure_weeks_of_month">
    <rdfs:label>weeks_of_month</rdfs:label>
    <rdfs:comment>Weeks during the month when maintenance should be performed. Weeks start on
the 1st, 8th, 15th, and 22nd days of the month, and have a duration of 7
days. Weeks start and end based on calendar dates, not days of the week.</rdfs:comment>
    <rdfs:domain rdf:resource="http://example.org/onto/class/google_oracle_database_cloud_exadata_infrastructure"/>
    <rdfs:range rdf:resource="http://www.w3.org/2001/XMLSchema#string"/>
  </owl:DatatypeProperty>
  <owl:DatatypeProperty rdf:about="http://example.org/onto/prop/google_oracle_database_cloud_exadata_infrastructure_create">
    <rdfs:label>create</rdfs:label>
    <rdfs:domain rdf:resource="http://example.org/onto/class/google_oracle_database_cloud_exadata_infrastructure"/>
    <rdfs:range rdf:resource="http://www.w3.org/2001/XMLSchema#string"/>
  </owl:DatatypeProperty>
  <owl:DatatypeProperty rdf:about="http://example.org/onto/prop/google_oracle_database_cloud_exadata_infrastructure_delete">
    <rdfs:label>delete</rdfs:label>
    <rdfs:domain rdf:resource="http://example.org/onto/class/google_oracle_database_cloud_exadata_infrastructure"/>
    <rdfs:range rdf:resource="http://www.w3.org/2001/XMLSchema#string"/>
  </owl:DatatypeProperty>
  <owl:DatatypeProperty rdf:about="http://example.org/onto/prop/google_oracle_database_cloud_exadata_infrastructure_update">
    <rdfs:label>update</rdfs:label>
    <rdfs:domain rdf:resource="http://example.org/onto/class/google_oracle_database_cloud_exadata_infrastructure"/>
    <rdfs:range rdf:resource="http://www.w3.org/2001/XMLSchema#string"/>
  </owl:DatatypeProperty>
</rdf:RDF>
