<?xml version="1.0" encoding="UTF-8"?>
<rdf:RDF
  xmlns:rdf="http://www.w3.org/1999/02/22-rdf-syntax-ns#"
  xmlns:rdfs="http://www.w3.org/2000/01/rdf-schema#"
  xmlns:owl="http://www.w3.org/2002/07/owl#"
  xmlns:xsd="http://www.w3.org/2001/XMLSchema#"
  xml:base="http://example.org/onto/">
  <owl:Class rdf:about="http://example.org/onto/class/google_network_security_mirroring_endpoint_group">
    <rdfs:label>google_network_security_mirroring_endpoint_group</rdfs:label>
    <rdfs:comment>#
#     ***     AUTO GENERATED CODE    ***    Type: MMv1     ***
#
# ----------------------------------------------------------------------------
#
#     This code is generated by Magic Modules using the following:
#
#     Configuration: https:#github.com/GoogleCloudPlatform/magic-modules/tree/main/mmv1/products/networksecurity/MirroringEndpointGroup.yaml
#     Template:      https:#github.com/GoogleCloudPlatform/magic-modules/tree/main/mmv1/templates/terraform/resource.html.markdown.tmpl
#
#     DO NOT EDIT this file directly. Any changes made to this file will be
#     overwritten during the next generation cycle.
#
# ----------------------------------------------------------------------------
subcategory: "Network Security"
description: |-
  An endpoint group is a consumer frontend for a deployment group (backend).
---</rdfs:comment>
  </owl:Class>
  <owl:DatatypeProperty rdf:about="http://example.org/onto/prop/google_network_security_mirroring_endpoint_group_associations">
    <rdfs:label>associations</rdfs:label>
    <rdfs:comment>List of associations to this endpoint group.</rdfs:comment>
    <rdfs:domain rdf:resource="http://example.org/onto/class/google_network_security_mirroring_endpoint_group"/>
    <rdfs:range rdf:resource="http://www.w3.org/2001/XMLSchema#string"/>
  </owl:DatatypeProperty>
  <owl:DatatypeProperty rdf:about="http://example.org/onto/prop/google_network_security_mirroring_endpoint_group_connected_deployment_groups">
    <rdfs:label>connected_deployment_groups</rdfs:label>
    <rdfs:comment>List of details about the connected deployment groups to this endpoint
group.</rdfs:comment>
    <rdfs:domain rdf:resource="http://example.org/onto/class/google_network_security_mirroring_endpoint_group"/>
    <rdfs:range rdf:resource="http://www.w3.org/2001/XMLSchema#string"/>
  </owl:DatatypeProperty>
  <owl:DatatypeProperty rdf:about="http://example.org/onto/prop/google_network_security_mirroring_endpoint_group_create_time">
    <rdfs:label>create_time</rdfs:label>
    <rdfs:comment>The timestamp when the resource was created.
See https://google.aip.dev/148#timestamps.</rdfs:comment>
    <rdfs:domain rdf:resource="http://example.org/onto/class/google_network_security_mirroring_endpoint_group"/>
    <rdfs:range rdf:resource="http://www.w3.org/2001/XMLSchema#string"/>
  </owl:DatatypeProperty>
  <owl:DatatypeProperty rdf:about="http://example.org/onto/prop/google_network_security_mirroring_endpoint_group_description">
    <rdfs:label>description</rdfs:label>
    <rdfs:comment>User-provided description of the endpoint group.
Used as additional context for the endpoint group.</rdfs:comment>
    <rdfs:domain rdf:resource="http://example.org/onto/class/google_network_security_mirroring_endpoint_group"/>
    <rdfs:range rdf:resource="http://www.w3.org/2001/XMLSchema#string"/>
  </owl:DatatypeProperty>
  <owl:DatatypeProperty rdf:about="http://example.org/onto/prop/google_network_security_mirroring_endpoint_group_effective_labels">
    <rdfs:label>effective_labels</rdfs:label>
    <rdfs:comment>All of labels (key/value pairs) present on the resource in GCP, including the labels configured through Terraform, other clients and services.</rdfs:comment>
    <rdfs:domain rdf:resource="http://example.org/onto/class/google_network_security_mirroring_endpoint_group"/>
    <rdfs:range rdf:resource="http://www.w3.org/2001/XMLSchema#string"/>
  </owl:DatatypeProperty>
  <owl:DatatypeProperty rdf:about="http://example.org/onto/prop/google_network_security_mirroring_endpoint_group_id">
    <rdfs:label>id</rdfs:label>
    <rdfs:domain rdf:resource="http://example.org/onto/class/google_network_security_mirroring_endpoint_group"/>
    <rdfs:range rdf:resource="http://www.w3.org/2001/XMLSchema#string"/>
  </owl:DatatypeProperty>
  <owl:DatatypeProperty rdf:about="http://example.org/onto/prop/google_network_security_mirroring_endpoint_group_labels">
    <rdfs:label>labels</rdfs:label>
    <rdfs:comment>Labels are key/value pairs that help to organize and filter resources.

**Note**: This field is non-authoritative, and will only manage the labels present in your configuration.
Please refer to the field 'effective_labels' for all of the labels present on the resource.</rdfs:comment>
    <rdfs:domain rdf:resource="http://example.org/onto/class/google_network_security_mirroring_endpoint_group"/>
    <rdfs:range rdf:resource="http://www.w3.org/2001/XMLSchema#string"/>
  </owl:DatatypeProperty>
  <owl:DatatypeProperty rdf:about="http://example.org/onto/prop/google_network_security_mirroring_endpoint_group_location">
    <rdfs:label>location</rdfs:label>
    <rdfs:comment>The cloud location of the endpoint group, currently restricted to 'global'.</rdfs:comment>
    <rdfs:domain rdf:resource="http://example.org/onto/class/google_network_security_mirroring_endpoint_group"/>
    <rdfs:range rdf:resource="http://www.w3.org/2001/XMLSchema#string"/>
  </owl:DatatypeProperty>
  <owl:DatatypeProperty rdf:about="http://example.org/onto/prop/google_network_security_mirroring_endpoint_group_mirroring_deployment_group">
    <rdfs:label>mirroring_deployment_group</rdfs:label>
    <rdfs:comment>The deployment group that this DIRECT endpoint group is connected to, for example:
'projects/123456789/locations/global/mirroringDeploymentGroups/my-dg'.
See https://google.aip.dev/124.</rdfs:comment>
    <rdfs:domain rdf:resource="http://example.org/onto/class/google_network_security_mirroring_endpoint_group"/>
    <rdfs:range rdf:resource="http://www.w3.org/2001/XMLSchema#string"/>
  </owl:DatatypeProperty>
  <owl:DatatypeProperty rdf:about="http://example.org/onto/prop/google_network_security_mirroring_endpoint_group_mirroring_endpoint_group_id">
    <rdfs:label>mirroring_endpoint_group_id</rdfs:label>
    <rdfs:comment>The ID to use for the endpoint group, which will become the final component
of the endpoint group's resource name.</rdfs:comment>
    <rdfs:domain rdf:resource="http://example.org/onto/class/google_network_security_mirroring_endpoint_group"/>
    <rdfs:range rdf:resource="http://www.w3.org/2001/XMLSchema#string"/>
  </owl:DatatypeProperty>
  <owl:DatatypeProperty rdf:about="http://example.org/onto/prop/google_network_security_mirroring_endpoint_group_name">
    <rdfs:label>name</rdfs:label>
    <rdfs:comment>The resource name of this endpoint group, for example:
'projects/123456789/locations/global/mirroringEndpointGroups/my-eg'.
See https://google.aip.dev/122 for more details.</rdfs:comment>
    <rdfs:domain rdf:resource="http://example.org/onto/class/google_network_security_mirroring_endpoint_group"/>
    <rdfs:range rdf:resource="http://www.w3.org/2001/XMLSchema#string"/>
  </owl:DatatypeProperty>
  <owl:DatatypeProperty rdf:about="http://example.org/onto/prop/google_network_security_mirroring_endpoint_group_project">
    <rdfs:label>project</rdfs:label>
    <rdfs:domain rdf:resource="http://example.org/onto/class/google_network_security_mirroring_endpoint_group"/>
    <rdfs:range rdf:resource="http://www.w3.org/2001/XMLSchema#string"/>
  </owl:DatatypeProperty>
  <owl:DatatypeProperty rdf:about="http://example.org/onto/prop/google_network_security_mirroring_endpoint_group_reconciling">
    <rdfs:label>reconciling</rdfs:label>
    <rdfs:comment>The current state of the resource does not match the user's intended state,
and the system is working to reconcile them. This is part of the normal
operation (e.g. adding a new association to the group).
See https://google.aip.dev/128.</rdfs:comment>
    <rdfs:domain rdf:resource="http://example.org/onto/class/google_network_security_mirroring_endpoint_group"/>
    <rdfs:range rdf:resource="http://www.w3.org/2001/XMLSchema#string"/>
  </owl:DatatypeProperty>
  <owl:DatatypeProperty rdf:about="http://example.org/onto/prop/google_network_security_mirroring_endpoint_group_state">
    <rdfs:label>state</rdfs:label>
    <rdfs:comment>The current state of the endpoint group.
See https://google.aip.dev/216.
Possible values:
STATE_UNSPECIFIED
ACTIVE
CLOSED
CREATING
DELETING
OUT_OF_SYNC
DELETE_FAILED</rdfs:comment>
    <rdfs:domain rdf:resource="http://example.org/onto/class/google_network_security_mirroring_endpoint_group"/>
    <rdfs:range rdf:resource="http://www.w3.org/2001/XMLSchema#string"/>
  </owl:DatatypeProperty>
  <owl:DatatypeProperty rdf:about="http://example.org/onto/prop/google_network_security_mirroring_endpoint_group_terraform_labels">
    <rdfs:label>terraform_labels</rdfs:label>
    <rdfs:comment>The combination of labels configured directly on the resource
 and default labels configured on the provider.</rdfs:comment>
    <rdfs:domain rdf:resource="http://example.org/onto/class/google_network_security_mirroring_endpoint_group"/>
    <rdfs:range rdf:resource="http://www.w3.org/2001/XMLSchema#string"/>
  </owl:DatatypeProperty>
  <owl:DatatypeProperty rdf:about="http://example.org/onto/prop/google_network_security_mirroring_endpoint_group_update_time">
    <rdfs:label>update_time</rdfs:label>
    <rdfs:comment>The timestamp when the resource was most recently updated.
See https://google.aip.dev/148#timestamps.</rdfs:comment>
    <rdfs:domain rdf:resource="http://example.org/onto/class/google_network_security_mirroring_endpoint_group"/>
    <rdfs:range rdf:resource="http://www.w3.org/2001/XMLSchema#string"/>
  </owl:DatatypeProperty>
  <owl:DatatypeProperty rdf:about="http://example.org/onto/prop/google_network_security_mirroring_endpoint_group_create">
    <rdfs:label>create</rdfs:label>
    <rdfs:domain rdf:resource="http://example.org/onto/class/google_network_security_mirroring_endpoint_group"/>
    <rdfs:range rdf:resource="http://www.w3.org/2001/XMLSchema#string"/>
  </owl:DatatypeProperty>
  <owl:DatatypeProperty rdf:about="http://example.org/onto/prop/google_network_security_mirroring_endpoint_group_delete">
    <rdfs:label>delete</rdfs:label>
    <rdfs:domain rdf:resource="http://example.org/onto/class/google_network_security_mirroring_endpoint_group"/>
    <rdfs:range rdf:resource="http://www.w3.org/2001/XMLSchema#string"/>
  </owl:DatatypeProperty>
  <owl:DatatypeProperty rdf:about="http://example.org/onto/prop/google_network_security_mirroring_endpoint_group_update">
    <rdfs:label>update</rdfs:label>
    <rdfs:domain rdf:resource="http://example.org/onto/class/google_network_security_mirroring_endpoint_group"/>
    <rdfs:range rdf:resource="http://www.w3.org/2001/XMLSchema#string"/>
  </owl:DatatypeProperty>
</rdf:RDF>
