<?xml version="1.0" encoding="UTF-8"?>
<rdf:RDF
  xmlns:rdf="http://www.w3.org/1999/02/22-rdf-syntax-ns#"
  xmlns:rdfs="http://www.w3.org/2000/01/rdf-schema#"
  xmlns:owl="http://www.w3.org/2002/07/owl#"
  xmlns:xsd="http://www.w3.org/2001/XMLSchema#"
  xml:base="http://example.org/onto/">
  <owl:Class rdf:about="http://example.org/onto/class/google_compute_region_disk">
    <rdfs:label>google_compute_region_disk</rdfs:label>
    <rdfs:comment>#
#     ***     AUTO GENERATED CODE    ***    Type: MMv1     ***
#
# ----------------------------------------------------------------------------
#
#     This code is generated by Magic Modules using the following:
#
#     Configuration: https:#github.com/GoogleCloudPlatform/magic-modules/tree/main/mmv1/products/compute/RegionDisk.yaml
#     Template:      https:#github.com/GoogleCloudPlatform/magic-modules/tree/main/mmv1/templates/terraform/resource.html.markdown.tmpl
#
#     DO NOT EDIT this file directly. Any changes made to this file will be
#     overwritten during the next generation cycle.
#
# ----------------------------------------------------------------------------
subcategory: "Compute Engine"
description: |-
  Persistent disks are durable storage devices that function similarly to
  the physical disks in a desktop or a server.
---</rdfs:comment>
  </owl:Class>
  <owl:DatatypeProperty rdf:about="http://example.org/onto/prop/google_compute_region_disk_access_mode">
    <rdfs:label>access_mode</rdfs:label>
    <rdfs:comment>The access mode of the disk.
For example:
  * READ_WRITE_SINGLE: The default AccessMode, means the disk can be attached to single instance in RW mode.
  * READ_WRITE_MANY: The AccessMode means the disk can be attached to multiple instances in RW mode.
  * READ_ONLY_SINGLE: The AccessMode means the disk can be attached to multiple instances in RO mode.
The AccessMode is only valid for Hyperdisk disk types.</rdfs:comment>
    <rdfs:domain rdf:resource="http://example.org/onto/class/google_compute_region_disk"/>
    <rdfs:range rdf:resource="http://www.w3.org/2001/XMLSchema#string"/>
  </owl:DatatypeProperty>
  <owl:DatatypeProperty rdf:about="http://example.org/onto/prop/google_compute_region_disk_create_snapshot_before_destroy">
    <rdfs:label>create_snapshot_before_destroy</rdfs:label>
    <rdfs:comment>If set to true, a snapshot of the disk will be created before it is destroyed.
If your disk is encrypted with customer managed encryption keys these will be reused for the snapshot creation.
The name of the snapshot by default will be '{{disk-name}}-YYYYMMDD-HHmm'</rdfs:comment>
    <rdfs:domain rdf:resource="http://example.org/onto/class/google_compute_region_disk"/>
    <rdfs:range rdf:resource="http://www.w3.org/2001/XMLSchema#string"/>
  </owl:DatatypeProperty>
  <owl:DatatypeProperty rdf:about="http://example.org/onto/prop/google_compute_region_disk_create_snapshot_before_destroy_prefix">
    <rdfs:label>create_snapshot_before_destroy_prefix</rdfs:label>
    <rdfs:comment>This will set a custom name prefix for the snapshot that's created when the disk is deleted.</rdfs:comment>
    <rdfs:domain rdf:resource="http://example.org/onto/class/google_compute_region_disk"/>
    <rdfs:range rdf:resource="http://www.w3.org/2001/XMLSchema#string"/>
  </owl:DatatypeProperty>
  <owl:DatatypeProperty rdf:about="http://example.org/onto/prop/google_compute_region_disk_creation_timestamp">
    <rdfs:label>creation_timestamp</rdfs:label>
    <rdfs:comment>Creation timestamp in RFC3339 text format.</rdfs:comment>
    <rdfs:domain rdf:resource="http://example.org/onto/class/google_compute_region_disk"/>
    <rdfs:range rdf:resource="http://www.w3.org/2001/XMLSchema#string"/>
  </owl:DatatypeProperty>
  <owl:DatatypeProperty rdf:about="http://example.org/onto/prop/google_compute_region_disk_description">
    <rdfs:label>description</rdfs:label>
    <rdfs:comment>An optional description of this resource. Provide this property when
you create the resource.</rdfs:comment>
    <rdfs:domain rdf:resource="http://example.org/onto/class/google_compute_region_disk"/>
    <rdfs:range rdf:resource="http://www.w3.org/2001/XMLSchema#string"/>
  </owl:DatatypeProperty>
  <owl:DatatypeProperty rdf:about="http://example.org/onto/prop/google_compute_region_disk_disk_id">
    <rdfs:label>disk_id</rdfs:label>
    <rdfs:comment>The unique identifier for the resource. This identifier is defined by the server.</rdfs:comment>
    <rdfs:domain rdf:resource="http://example.org/onto/class/google_compute_region_disk"/>
    <rdfs:range rdf:resource="http://www.w3.org/2001/XMLSchema#string"/>
  </owl:DatatypeProperty>
  <owl:DatatypeProperty rdf:about="http://example.org/onto/prop/google_compute_region_disk_effective_labels">
    <rdfs:label>effective_labels</rdfs:label>
    <rdfs:comment>All of labels (key/value pairs) present on the resource in GCP, including the labels configured through Terraform, other clients and services.</rdfs:comment>
    <rdfs:domain rdf:resource="http://example.org/onto/class/google_compute_region_disk"/>
    <rdfs:range rdf:resource="http://www.w3.org/2001/XMLSchema#string"/>
  </owl:DatatypeProperty>
  <owl:DatatypeProperty rdf:about="http://example.org/onto/prop/google_compute_region_disk_id">
    <rdfs:label>id</rdfs:label>
    <rdfs:domain rdf:resource="http://example.org/onto/class/google_compute_region_disk"/>
    <rdfs:range rdf:resource="http://www.w3.org/2001/XMLSchema#string"/>
  </owl:DatatypeProperty>
  <owl:DatatypeProperty rdf:about="http://example.org/onto/prop/google_compute_region_disk_label_fingerprint">
    <rdfs:label>label_fingerprint</rdfs:label>
    <rdfs:comment>The fingerprint used for optimistic locking of this resource.  Used
internally during updates.</rdfs:comment>
    <rdfs:domain rdf:resource="http://example.org/onto/class/google_compute_region_disk"/>
    <rdfs:range rdf:resource="http://www.w3.org/2001/XMLSchema#string"/>
  </owl:DatatypeProperty>
  <owl:DatatypeProperty rdf:about="http://example.org/onto/prop/google_compute_region_disk_labels">
    <rdfs:label>labels</rdfs:label>
    <rdfs:comment>Labels to apply to this disk.  A list of key->value pairs.


**Note**: This field is non-authoritative, and will only manage the labels present in your configuration.
Please refer to the field 'effective_labels' for all of the labels present on the resource.</rdfs:comment>
    <rdfs:domain rdf:resource="http://example.org/onto/class/google_compute_region_disk"/>
    <rdfs:range rdf:resource="http://www.w3.org/2001/XMLSchema#string"/>
  </owl:DatatypeProperty>
  <owl:DatatypeProperty rdf:about="http://example.org/onto/prop/google_compute_region_disk_last_attach_timestamp">
    <rdfs:label>last_attach_timestamp</rdfs:label>
    <rdfs:comment>Last attach timestamp in RFC3339 text format.</rdfs:comment>
    <rdfs:domain rdf:resource="http://example.org/onto/class/google_compute_region_disk"/>
    <rdfs:range rdf:resource="http://www.w3.org/2001/XMLSchema#string"/>
  </owl:DatatypeProperty>
  <owl:DatatypeProperty rdf:about="http://example.org/onto/prop/google_compute_region_disk_last_detach_timestamp">
    <rdfs:label>last_detach_timestamp</rdfs:label>
    <rdfs:comment>Last detach timestamp in RFC3339 text format.</rdfs:comment>
    <rdfs:domain rdf:resource="http://example.org/onto/class/google_compute_region_disk"/>
    <rdfs:range rdf:resource="http://www.w3.org/2001/XMLSchema#string"/>
  </owl:DatatypeProperty>
  <owl:DatatypeProperty rdf:about="http://example.org/onto/prop/google_compute_region_disk_licenses">
    <rdfs:label>licenses</rdfs:label>
    <rdfs:comment>Any applicable license URI.</rdfs:comment>
    <rdfs:domain rdf:resource="http://example.org/onto/class/google_compute_region_disk"/>
    <rdfs:range rdf:resource="http://www.w3.org/2001/XMLSchema#string"/>
  </owl:DatatypeProperty>
  <owl:DatatypeProperty rdf:about="http://example.org/onto/prop/google_compute_region_disk_name">
    <rdfs:label>name</rdfs:label>
    <rdfs:comment>Name of the resource. Provided by the client when the resource is
created. The name must be 1-63 characters long, and comply with
RFC1035. Specifically, the name must be 1-63 characters long and match
the regular expression '[a-z]([-a-z0-9]*[a-z0-9])?' which means the
first character must be a lowercase letter, and all following
characters must be a dash, lowercase letter, or digit, except the last
character, which cannot be a dash.</rdfs:comment>
    <rdfs:domain rdf:resource="http://example.org/onto/class/google_compute_region_disk"/>
    <rdfs:range rdf:resource="http://www.w3.org/2001/XMLSchema#string"/>
  </owl:DatatypeProperty>
  <owl:DatatypeProperty rdf:about="http://example.org/onto/prop/google_compute_region_disk_physical_block_size_bytes">
    <rdfs:label>physical_block_size_bytes</rdfs:label>
    <rdfs:comment>Physical block size of the persistent disk, in bytes. If not present
in a request, a default value is used. Currently supported sizes
are 4096 and 16384, other sizes may be added in the future.
If an unsupported value is requested, the error message will list
the supported values for the caller's project.</rdfs:comment>
    <rdfs:domain rdf:resource="http://example.org/onto/class/google_compute_region_disk"/>
    <rdfs:range rdf:resource="http://www.w3.org/2001/XMLSchema#string"/>
  </owl:DatatypeProperty>
  <owl:DatatypeProperty rdf:about="http://example.org/onto/prop/google_compute_region_disk_project">
    <rdfs:label>project</rdfs:label>
    <rdfs:domain rdf:resource="http://example.org/onto/class/google_compute_region_disk"/>
    <rdfs:range rdf:resource="http://www.w3.org/2001/XMLSchema#string"/>
  </owl:DatatypeProperty>
  <owl:DatatypeProperty rdf:about="http://example.org/onto/prop/google_compute_region_disk_provisioned_iops">
    <rdfs:label>provisioned_iops</rdfs:label>
    <rdfs:comment>Indicates how many IOPS to provision for the disk. This sets the number of I/O operations per second
that the disk can handle. Values must be between 10,000 and 120,000.
For more details, see the Extreme persistent disk [documentation](https://cloud.google.com/compute/docs/disks/extreme-persistent-disk).</rdfs:comment>
    <rdfs:domain rdf:resource="http://example.org/onto/class/google_compute_region_disk"/>
    <rdfs:range rdf:resource="http://www.w3.org/2001/XMLSchema#string"/>
  </owl:DatatypeProperty>
  <owl:DatatypeProperty rdf:about="http://example.org/onto/prop/google_compute_region_disk_provisioned_throughput">
    <rdfs:label>provisioned_throughput</rdfs:label>
    <rdfs:comment>Indicates how much throughput to provision for the disk. This sets the number of throughput
mb per second that the disk can handle. Values must be greater than or equal to 1.</rdfs:comment>
    <rdfs:domain rdf:resource="http://example.org/onto/class/google_compute_region_disk"/>
    <rdfs:range rdf:resource="http://www.w3.org/2001/XMLSchema#string"/>
  </owl:DatatypeProperty>
  <owl:DatatypeProperty rdf:about="http://example.org/onto/prop/google_compute_region_disk_region">
    <rdfs:label>region</rdfs:label>
    <rdfs:comment>A reference to the region where the disk resides.</rdfs:comment>
    <rdfs:domain rdf:resource="http://example.org/onto/class/google_compute_region_disk"/>
    <rdfs:range rdf:resource="http://www.w3.org/2001/XMLSchema#string"/>
  </owl:DatatypeProperty>
  <owl:DatatypeProperty rdf:about="http://example.org/onto/prop/google_compute_region_disk_replica_zones">
    <rdfs:label>replica_zones</rdfs:label>
    <rdfs:comment>URLs of the zones where the disk should be replicated to.</rdfs:comment>
    <rdfs:domain rdf:resource="http://example.org/onto/class/google_compute_region_disk"/>
    <rdfs:range rdf:resource="http://www.w3.org/2001/XMLSchema#string"/>
  </owl:DatatypeProperty>
  <owl:DatatypeProperty rdf:about="http://example.org/onto/prop/google_compute_region_disk_self_link">
    <rdfs:label>self_link</rdfs:label>
    <rdfs:domain rdf:resource="http://example.org/onto/class/google_compute_region_disk"/>
    <rdfs:range rdf:resource="http://www.w3.org/2001/XMLSchema#string"/>
  </owl:DatatypeProperty>
  <owl:DatatypeProperty rdf:about="http://example.org/onto/prop/google_compute_region_disk_size">
    <rdfs:label>size</rdfs:label>
    <rdfs:comment>Size of the persistent disk, specified in GB. You can specify this
field when creating a persistent disk using the sourceImage or
sourceSnapshot parameter, or specify it alone to create an empty
persistent disk.

If you specify this field along with sourceImage or sourceSnapshot,
the value of sizeGb must not be less than the size of the sourceImage
or the size of the snapshot.</rdfs:comment>
    <rdfs:domain rdf:resource="http://example.org/onto/class/google_compute_region_disk"/>
    <rdfs:range rdf:resource="http://www.w3.org/2001/XMLSchema#string"/>
  </owl:DatatypeProperty>
  <owl:DatatypeProperty rdf:about="http://example.org/onto/prop/google_compute_region_disk_snapshot">
    <rdfs:label>snapshot</rdfs:label>
    <rdfs:comment>The source snapshot used to create this disk. You can provide this as
a partial or full URL to the resource. For example, the following are
valid values:

* 'https://www.googleapis.com/compute/v1/projects/project/global/snapshots/snapshot'
* 'projects/project/global/snapshots/snapshot'
* 'global/snapshots/snapshot'
* 'snapshot'</rdfs:comment>
    <rdfs:domain rdf:resource="http://example.org/onto/class/google_compute_region_disk"/>
    <rdfs:range rdf:resource="http://www.w3.org/2001/XMLSchema#string"/>
  </owl:DatatypeProperty>
  <owl:DatatypeProperty rdf:about="http://example.org/onto/prop/google_compute_region_disk_source_disk">
    <rdfs:label>source_disk</rdfs:label>
    <rdfs:comment>The source disk used to create this disk. You can provide this as a partial or full URL to the resource.
For example, the following are valid values:

* https://www.googleapis.com/compute/v1/projects/{project}/zones/{zone}/disks/{disk}
* https://www.googleapis.com/compute/v1/projects/{project}/regions/{region}/disks/{disk}
* projects/{project}/zones/{zone}/disks/{disk}
* projects/{project}/regions/{region}/disks/{disk}
* zones/{zone}/disks/{disk}
* regions/{region}/disks/{disk}</rdfs:comment>
    <rdfs:domain rdf:resource="http://example.org/onto/class/google_compute_region_disk"/>
    <rdfs:range rdf:resource="http://www.w3.org/2001/XMLSchema#string"/>
  </owl:DatatypeProperty>
  <owl:DatatypeProperty rdf:about="http://example.org/onto/prop/google_compute_region_disk_source_disk_id">
    <rdfs:label>source_disk_id</rdfs:label>
    <rdfs:comment>The ID value of the disk used to create this image. This value may
be used to determine whether the image was taken from the current
or a previous instance of a given disk name.</rdfs:comment>
    <rdfs:domain rdf:resource="http://example.org/onto/class/google_compute_region_disk"/>
    <rdfs:range rdf:resource="http://www.w3.org/2001/XMLSchema#string"/>
  </owl:DatatypeProperty>
  <owl:DatatypeProperty rdf:about="http://example.org/onto/prop/google_compute_region_disk_source_snapshot_id">
    <rdfs:label>source_snapshot_id</rdfs:label>
    <rdfs:comment>The unique ID of the snapshot used to create this disk. This value
identifies the exact snapshot that was used to create this persistent
disk. For example, if you created the persistent disk from a snapshot
that was later deleted and recreated under the same name, the source
snapshot ID would identify the exact version of the snapshot that was
used.</rdfs:comment>
    <rdfs:domain rdf:resource="http://example.org/onto/class/google_compute_region_disk"/>
    <rdfs:range rdf:resource="http://www.w3.org/2001/XMLSchema#string"/>
  </owl:DatatypeProperty>
  <owl:DatatypeProperty rdf:about="http://example.org/onto/prop/google_compute_region_disk_terraform_labels">
    <rdfs:label>terraform_labels</rdfs:label>
    <rdfs:comment>The combination of labels configured directly on the resource
 and default labels configured on the provider.</rdfs:comment>
    <rdfs:domain rdf:resource="http://example.org/onto/class/google_compute_region_disk"/>
    <rdfs:range rdf:resource="http://www.w3.org/2001/XMLSchema#string"/>
  </owl:DatatypeProperty>
  <owl:DatatypeProperty rdf:about="http://example.org/onto/prop/google_compute_region_disk_type">
    <rdfs:label>type</rdfs:label>
    <rdfs:comment>URL of the disk type resource describing which disk type to use to
create the disk. Provide this when creating the disk.</rdfs:comment>
    <rdfs:domain rdf:resource="http://example.org/onto/class/google_compute_region_disk"/>
    <rdfs:range rdf:resource="http://www.w3.org/2001/XMLSchema#string"/>
  </owl:DatatypeProperty>
  <owl:DatatypeProperty rdf:about="http://example.org/onto/prop/google_compute_region_disk_users">
    <rdfs:label>users</rdfs:label>
    <rdfs:comment>Links to the users of the disk (attached instances) in form:
project/zones/zone/instances/instance</rdfs:comment>
    <rdfs:domain rdf:resource="http://example.org/onto/class/google_compute_region_disk"/>
    <rdfs:range rdf:resource="http://www.w3.org/2001/XMLSchema#string"/>
  </owl:DatatypeProperty>
  <owl:DatatypeProperty rdf:about="http://example.org/onto/prop/google_compute_region_disk_disk">
    <rdfs:label>disk</rdfs:label>
    <rdfs:comment>Primary disk for asynchronous disk replication.</rdfs:comment>
    <rdfs:domain rdf:resource="http://example.org/onto/class/google_compute_region_disk"/>
    <rdfs:range rdf:resource="http://www.w3.org/2001/XMLSchema#string"/>
  </owl:DatatypeProperty>
  <owl:DatatypeProperty rdf:about="http://example.org/onto/prop/google_compute_region_disk_kms_key_name">
    <rdfs:label>kms_key_name</rdfs:label>
    <rdfs:comment>The name of the encryption key that is stored in Google Cloud KMS.</rdfs:comment>
    <rdfs:domain rdf:resource="http://example.org/onto/class/google_compute_region_disk"/>
    <rdfs:range rdf:resource="http://www.w3.org/2001/XMLSchema#string"/>
  </owl:DatatypeProperty>
  <owl:DatatypeProperty rdf:about="http://example.org/onto/prop/google_compute_region_disk_raw_key">
    <rdfs:label>raw_key</rdfs:label>
    <rdfs:comment>Specifies a 256-bit customer-supplied encryption key, encoded in
RFC 4648 base64 to either encrypt or decrypt this resource.</rdfs:comment>
    <rdfs:domain rdf:resource="http://example.org/onto/class/google_compute_region_disk"/>
    <rdfs:range rdf:resource="http://www.w3.org/2001/XMLSchema#string"/>
  </owl:DatatypeProperty>
  <owl:DatatypeProperty rdf:about="http://example.org/onto/prop/google_compute_region_disk_rsa_encrypted_key">
    <rdfs:label>rsa_encrypted_key</rdfs:label>
    <rdfs:comment>Specifies an RFC 4648 base64 encoded, RSA-wrapped 2048-bit
customer-supplied encryption key to either encrypt or decrypt
this resource. You can provide either the rawKey or the rsaEncryptedKey.</rdfs:comment>
    <rdfs:domain rdf:resource="http://example.org/onto/class/google_compute_region_disk"/>
    <rdfs:range rdf:resource="http://www.w3.org/2001/XMLSchema#string"/>
  </owl:DatatypeProperty>
  <owl:DatatypeProperty rdf:about="http://example.org/onto/prop/google_compute_region_disk_sha256">
    <rdfs:label>sha256</rdfs:label>
    <rdfs:comment>The RFC 4648 base64 encoded SHA-256 hash of the customer-supplied
encryption key that protects this resource.</rdfs:comment>
    <rdfs:domain rdf:resource="http://example.org/onto/class/google_compute_region_disk"/>
    <rdfs:range rdf:resource="http://www.w3.org/2001/XMLSchema#string"/>
  </owl:DatatypeProperty>
  <owl:DatatypeProperty rdf:about="http://example.org/onto/prop/google_compute_region_disk_type">
    <rdfs:label>type</rdfs:label>
    <rdfs:comment>The type of supported feature. Read [Enabling guest operating system features](https://cloud.google.com/compute/docs/images/create-delete-deprecate-private-images#guest-os-features) to see a list of available options. Possible values: ["MULTI_IP_SUBNET", "SECURE_BOOT", "SEV_CAPABLE", "UEFI_COMPATIBLE", "VIRTIO_SCSI_MULTIQUEUE", "WINDOWS", "GVNIC", "SEV_LIVE_MIGRATABLE", "SEV_SNP_CAPABLE", "SUSPEND_RESUME_COMPATIBLE", "TDX_CAPABLE"]</rdfs:comment>
    <rdfs:domain rdf:resource="http://example.org/onto/class/google_compute_region_disk"/>
    <rdfs:range rdf:resource="http://www.w3.org/2001/XMLSchema#string"/>
  </owl:DatatypeProperty>
  <owl:DatatypeProperty rdf:about="http://example.org/onto/prop/google_compute_region_disk_raw_key">
    <rdfs:label>raw_key</rdfs:label>
    <rdfs:comment>Specifies a 256-bit customer-supplied encryption key, encoded in
RFC 4648 base64 to either encrypt or decrypt this resource.</rdfs:comment>
    <rdfs:domain rdf:resource="http://example.org/onto/class/google_compute_region_disk"/>
    <rdfs:range rdf:resource="http://www.w3.org/2001/XMLSchema#string"/>
  </owl:DatatypeProperty>
  <owl:DatatypeProperty rdf:about="http://example.org/onto/prop/google_compute_region_disk_sha256">
    <rdfs:label>sha256</rdfs:label>
    <rdfs:comment>The RFC 4648 base64 encoded SHA-256 hash of the customer-supplied
encryption key that protects this resource.</rdfs:comment>
    <rdfs:domain rdf:resource="http://example.org/onto/class/google_compute_region_disk"/>
    <rdfs:range rdf:resource="http://www.w3.org/2001/XMLSchema#string"/>
  </owl:DatatypeProperty>
  <owl:DatatypeProperty rdf:about="http://example.org/onto/prop/google_compute_region_disk_create">
    <rdfs:label>create</rdfs:label>
    <rdfs:domain rdf:resource="http://example.org/onto/class/google_compute_region_disk"/>
    <rdfs:range rdf:resource="http://www.w3.org/2001/XMLSchema#string"/>
  </owl:DatatypeProperty>
  <owl:DatatypeProperty rdf:about="http://example.org/onto/prop/google_compute_region_disk_delete">
    <rdfs:label>delete</rdfs:label>
    <rdfs:domain rdf:resource="http://example.org/onto/class/google_compute_region_disk"/>
    <rdfs:range rdf:resource="http://www.w3.org/2001/XMLSchema#string"/>
  </owl:DatatypeProperty>
  <owl:DatatypeProperty rdf:about="http://example.org/onto/prop/google_compute_region_disk_update">
    <rdfs:label>update</rdfs:label>
    <rdfs:domain rdf:resource="http://example.org/onto/class/google_compute_region_disk"/>
    <rdfs:range rdf:resource="http://www.w3.org/2001/XMLSchema#string"/>
  </owl:DatatypeProperty>
</rdf:RDF>
