<?xml version="1.0" encoding="UTF-8"?>
<rdf:RDF
  xmlns:rdf="http://www.w3.org/1999/02/22-rdf-syntax-ns#"
  xmlns:rdfs="http://www.w3.org/2000/01/rdf-schema#"
  xmlns:owl="http://www.w3.org/2002/07/owl#"
  xmlns:xsd="http://www.w3.org/2001/XMLSchema#"
  xml:base="http://example.org/onto/">
  <owl:Class rdf:about="http://example.org/onto/class/google_iam_deny_policy">
    <rdfs:label>google_iam_deny_policy</rdfs:label>
    <rdfs:comment>#
#     ***     AUTO GENERATED CODE    ***    Type: MMv1     ***
#
# ----------------------------------------------------------------------------
#
#     This code is generated by Magic Modules using the following:
#
#     Configuration: https:#github.com/GoogleCloudPlatform/magic-modules/tree/main/mmv1/products/iam2/DenyPolicy.yaml
#     Template:      https:#github.com/GoogleCloudPlatform/magic-modules/tree/main/mmv1/templates/terraform/resource.html.markdown.tmpl
#
#     DO NOT EDIT this file directly. Any changes made to this file will be
#     overwritten during the next generation cycle.
#
# ----------------------------------------------------------------------------
subcategory: "Cloud IAM"
description: |-
  Represents a collection of denial policies to apply to a given resource.
---</rdfs:comment>
  </owl:Class>
  <owl:DatatypeProperty rdf:about="http://example.org/onto/prop/google_iam_deny_policy_display_name">
    <rdfs:label>display_name</rdfs:label>
    <rdfs:comment>The display name of the rule.</rdfs:comment>
    <rdfs:domain rdf:resource="http://example.org/onto/class/google_iam_deny_policy"/>
    <rdfs:range rdf:resource="http://www.w3.org/2001/XMLSchema#string"/>
  </owl:DatatypeProperty>
  <owl:DatatypeProperty rdf:about="http://example.org/onto/prop/google_iam_deny_policy_etag">
    <rdfs:label>etag</rdfs:label>
    <rdfs:comment>The hash of the resource. Used internally during updates.</rdfs:comment>
    <rdfs:domain rdf:resource="http://example.org/onto/class/google_iam_deny_policy"/>
    <rdfs:range rdf:resource="http://www.w3.org/2001/XMLSchema#string"/>
  </owl:DatatypeProperty>
  <owl:DatatypeProperty rdf:about="http://example.org/onto/prop/google_iam_deny_policy_id">
    <rdfs:label>id</rdfs:label>
    <rdfs:domain rdf:resource="http://example.org/onto/class/google_iam_deny_policy"/>
    <rdfs:range rdf:resource="http://www.w3.org/2001/XMLSchema#string"/>
  </owl:DatatypeProperty>
  <owl:DatatypeProperty rdf:about="http://example.org/onto/prop/google_iam_deny_policy_name">
    <rdfs:label>name</rdfs:label>
    <rdfs:comment>The name of the policy.</rdfs:comment>
    <rdfs:domain rdf:resource="http://example.org/onto/class/google_iam_deny_policy"/>
    <rdfs:range rdf:resource="http://www.w3.org/2001/XMLSchema#string"/>
  </owl:DatatypeProperty>
  <owl:DatatypeProperty rdf:about="http://example.org/onto/prop/google_iam_deny_policy_parent">
    <rdfs:label>parent</rdfs:label>
    <rdfs:comment>The attachment point is identified by its URL-encoded full resource name.</rdfs:comment>
    <rdfs:domain rdf:resource="http://example.org/onto/class/google_iam_deny_policy"/>
    <rdfs:range rdf:resource="http://www.w3.org/2001/XMLSchema#string"/>
  </owl:DatatypeProperty>
  <owl:DatatypeProperty rdf:about="http://example.org/onto/prop/google_iam_deny_policy_description">
    <rdfs:label>description</rdfs:label>
    <rdfs:comment>The description of the rule.</rdfs:comment>
    <rdfs:domain rdf:resource="http://example.org/onto/class/google_iam_deny_policy"/>
    <rdfs:range rdf:resource="http://www.w3.org/2001/XMLSchema#string"/>
  </owl:DatatypeProperty>
  <owl:DatatypeProperty rdf:about="http://example.org/onto/prop/google_iam_deny_policy_denied_permissions">
    <rdfs:label>denied_permissions</rdfs:label>
    <rdfs:comment>The permissions that are explicitly denied by this rule. Each permission uses the format '{service-fqdn}/{resource}.{verb}',
where '{service-fqdn}' is the fully qualified domain name for the service. For example, 'iam.googleapis.com/roles.list'.</rdfs:comment>
    <rdfs:domain rdf:resource="http://example.org/onto/class/google_iam_deny_policy"/>
    <rdfs:range rdf:resource="http://www.w3.org/2001/XMLSchema#string"/>
  </owl:DatatypeProperty>
  <owl:DatatypeProperty rdf:about="http://example.org/onto/prop/google_iam_deny_policy_denied_principals">
    <rdfs:label>denied_principals</rdfs:label>
    <rdfs:comment>The identities that are prevented from using one or more permissions on Google Cloud resources.</rdfs:comment>
    <rdfs:domain rdf:resource="http://example.org/onto/class/google_iam_deny_policy"/>
    <rdfs:range rdf:resource="http://www.w3.org/2001/XMLSchema#string"/>
  </owl:DatatypeProperty>
  <owl:DatatypeProperty rdf:about="http://example.org/onto/prop/google_iam_deny_policy_exception_permissions">
    <rdfs:label>exception_permissions</rdfs:label>
    <rdfs:comment>Specifies the permissions that this rule excludes from the set of denied permissions given by deniedPermissions.
If a permission appears in deniedPermissions and in exceptionPermissions then it will not be denied.
The excluded permissions can be specified using the same syntax as deniedPermissions.</rdfs:comment>
    <rdfs:domain rdf:resource="http://example.org/onto/class/google_iam_deny_policy"/>
    <rdfs:range rdf:resource="http://www.w3.org/2001/XMLSchema#string"/>
  </owl:DatatypeProperty>
  <owl:DatatypeProperty rdf:about="http://example.org/onto/prop/google_iam_deny_policy_exception_principals">
    <rdfs:label>exception_principals</rdfs:label>
    <rdfs:comment>The identities that are excluded from the deny rule, even if they are listed in the deniedPrincipals.
For example, you could add a Google group to the deniedPrincipals, then exclude specific users who belong to that group.</rdfs:comment>
    <rdfs:domain rdf:resource="http://example.org/onto/class/google_iam_deny_policy"/>
    <rdfs:range rdf:resource="http://www.w3.org/2001/XMLSchema#string"/>
  </owl:DatatypeProperty>
  <owl:DatatypeProperty rdf:about="http://example.org/onto/prop/google_iam_deny_policy_description">
    <rdfs:label>description</rdfs:label>
    <rdfs:comment>Description of the expression. This is a longer text which describes the expression,
e.g. when hovered over it in a UI.</rdfs:comment>
    <rdfs:domain rdf:resource="http://example.org/onto/class/google_iam_deny_policy"/>
    <rdfs:range rdf:resource="http://www.w3.org/2001/XMLSchema#string"/>
  </owl:DatatypeProperty>
  <owl:DatatypeProperty rdf:about="http://example.org/onto/prop/google_iam_deny_policy_expression">
    <rdfs:label>expression</rdfs:label>
    <rdfs:comment>Textual representation of an expression in Common Expression Language syntax.</rdfs:comment>
    <rdfs:domain rdf:resource="http://example.org/onto/class/google_iam_deny_policy"/>
    <rdfs:range rdf:resource="http://www.w3.org/2001/XMLSchema#string"/>
  </owl:DatatypeProperty>
  <owl:DatatypeProperty rdf:about="http://example.org/onto/prop/google_iam_deny_policy_location">
    <rdfs:label>location</rdfs:label>
    <rdfs:comment>String indicating the location of the expression for error reporting,
e.g. a file name and a position in the file.</rdfs:comment>
    <rdfs:domain rdf:resource="http://example.org/onto/class/google_iam_deny_policy"/>
    <rdfs:range rdf:resource="http://www.w3.org/2001/XMLSchema#string"/>
  </owl:DatatypeProperty>
  <owl:DatatypeProperty rdf:about="http://example.org/onto/prop/google_iam_deny_policy_title">
    <rdfs:label>title</rdfs:label>
    <rdfs:comment>Title for the expression, i.e. a short string describing its purpose.
This can be used e.g. in UIs which allow to enter the expression.</rdfs:comment>
    <rdfs:domain rdf:resource="http://example.org/onto/class/google_iam_deny_policy"/>
    <rdfs:range rdf:resource="http://www.w3.org/2001/XMLSchema#string"/>
  </owl:DatatypeProperty>
  <owl:DatatypeProperty rdf:about="http://example.org/onto/prop/google_iam_deny_policy_create">
    <rdfs:label>create</rdfs:label>
    <rdfs:domain rdf:resource="http://example.org/onto/class/google_iam_deny_policy"/>
    <rdfs:range rdf:resource="http://www.w3.org/2001/XMLSchema#string"/>
  </owl:DatatypeProperty>
  <owl:DatatypeProperty rdf:about="http://example.org/onto/prop/google_iam_deny_policy_delete">
    <rdfs:label>delete</rdfs:label>
    <rdfs:domain rdf:resource="http://example.org/onto/class/google_iam_deny_policy"/>
    <rdfs:range rdf:resource="http://www.w3.org/2001/XMLSchema#string"/>
  </owl:DatatypeProperty>
  <owl:DatatypeProperty rdf:about="http://example.org/onto/prop/google_iam_deny_policy_update">
    <rdfs:label>update</rdfs:label>
    <rdfs:domain rdf:resource="http://example.org/onto/class/google_iam_deny_policy"/>
    <rdfs:range rdf:resource="http://www.w3.org/2001/XMLSchema#string"/>
  </owl:DatatypeProperty>
</rdf:RDF>
