<?xml version="1.0" encoding="UTF-8"?>
<rdf:RDF
  xmlns:rdf="http://www.w3.org/1999/02/22-rdf-syntax-ns#"
  xmlns:rdfs="http://www.w3.org/2000/01/rdf-schema#"
  xmlns:owl="http://www.w3.org/2002/07/owl#"
  xmlns:xsd="http://www.w3.org/2001/XMLSchema#"
  xml:base="http://example.org/onto/">
  <owl:Class rdf:about="http://example.org/onto/class/google_cloud_run_domain_mapping">
    <rdfs:label>google_cloud_run_domain_mapping</rdfs:label>
    <rdfs:comment>#
#     ***     AUTO GENERATED CODE    ***    Type: MMv1     ***
#
# ----------------------------------------------------------------------------
#
#     This code is generated by Magic Modules using the following:
#
#     Configuration: https:#github.com/GoogleCloudPlatform/magic-modules/tree/main/mmv1/products/cloudrun/DomainMapping.yaml
#     Template:      https:#github.com/GoogleCloudPlatform/magic-modules/tree/main/mmv1/templates/terraform/resource.html.markdown.tmpl
#
#     DO NOT EDIT this file directly. Any changes made to this file will be
#     overwritten during the next generation cycle.
#
# ----------------------------------------------------------------------------
subcategory: "Cloud Run"
description: |-
  Resource to hold the state and status of a user's domain mapping.
---</rdfs:comment>
  </owl:Class>
  <owl:DatatypeProperty rdf:about="http://example.org/onto/prop/google_cloud_run_domain_mapping_id">
    <rdfs:label>id</rdfs:label>
    <rdfs:domain rdf:resource="http://example.org/onto/class/google_cloud_run_domain_mapping"/>
    <rdfs:range rdf:resource="http://www.w3.org/2001/XMLSchema#string"/>
  </owl:DatatypeProperty>
  <owl:DatatypeProperty rdf:about="http://example.org/onto/prop/google_cloud_run_domain_mapping_location">
    <rdfs:label>location</rdfs:label>
    <rdfs:comment>The location of the cloud run instance. eg us-central1</rdfs:comment>
    <rdfs:domain rdf:resource="http://example.org/onto/class/google_cloud_run_domain_mapping"/>
    <rdfs:range rdf:resource="http://www.w3.org/2001/XMLSchema#string"/>
  </owl:DatatypeProperty>
  <owl:DatatypeProperty rdf:about="http://example.org/onto/prop/google_cloud_run_domain_mapping_name">
    <rdfs:label>name</rdfs:label>
    <rdfs:comment>Name should be a [verified](https://support.google.com/webmasters/answer/9008080) domain</rdfs:comment>
    <rdfs:domain rdf:resource="http://example.org/onto/class/google_cloud_run_domain_mapping"/>
    <rdfs:range rdf:resource="http://www.w3.org/2001/XMLSchema#string"/>
  </owl:DatatypeProperty>
  <owl:DatatypeProperty rdf:about="http://example.org/onto/prop/google_cloud_run_domain_mapping_project">
    <rdfs:label>project</rdfs:label>
    <rdfs:domain rdf:resource="http://example.org/onto/class/google_cloud_run_domain_mapping"/>
    <rdfs:range rdf:resource="http://www.w3.org/2001/XMLSchema#string"/>
  </owl:DatatypeProperty>
  <owl:DatatypeProperty rdf:about="http://example.org/onto/prop/google_cloud_run_domain_mapping_status">
    <rdfs:label>status</rdfs:label>
    <rdfs:comment>The current status of the DomainMapping.</rdfs:comment>
    <rdfs:domain rdf:resource="http://example.org/onto/class/google_cloud_run_domain_mapping"/>
    <rdfs:range rdf:resource="http://www.w3.org/2001/XMLSchema#string"/>
  </owl:DatatypeProperty>
  <owl:DatatypeProperty rdf:about="http://example.org/onto/prop/google_cloud_run_domain_mapping_annotations">
    <rdfs:label>annotations</rdfs:label>
    <rdfs:comment>Annotations is a key value map stored with a resource that
may be set by external tools to store and retrieve arbitrary metadata.
More info: https://kubernetes.io/docs/concepts/overview/working-with-objects/annotations

**Note**: The Cloud Run API may add additional annotations that were not provided in your config.
If terraform plan shows a diff where a server-side annotation is added, you can add it to your config
or apply the lifecycle.ignore_changes rule to the metadata.0.annotations field.

**Note**: This field is non-authoritative, and will only manage the annotations present in your configuration.
Please refer to the field 'effective_annotations' for all of the annotations present on the resource.</rdfs:comment>
    <rdfs:domain rdf:resource="http://example.org/onto/class/google_cloud_run_domain_mapping"/>
    <rdfs:range rdf:resource="http://www.w3.org/2001/XMLSchema#string"/>
  </owl:DatatypeProperty>
  <owl:DatatypeProperty rdf:about="http://example.org/onto/prop/google_cloud_run_domain_mapping_effective_annotations">
    <rdfs:label>effective_annotations</rdfs:label>
    <rdfs:comment>All of annotations (key/value pairs) present on the resource in GCP, including the annotations configured through Terraform, other clients and services.</rdfs:comment>
    <rdfs:domain rdf:resource="http://example.org/onto/class/google_cloud_run_domain_mapping"/>
    <rdfs:range rdf:resource="http://www.w3.org/2001/XMLSchema#string"/>
  </owl:DatatypeProperty>
  <owl:DatatypeProperty rdf:about="http://example.org/onto/prop/google_cloud_run_domain_mapping_effective_labels">
    <rdfs:label>effective_labels</rdfs:label>
    <rdfs:comment>All of labels (key/value pairs) present on the resource in GCP, including the labels configured through Terraform, other clients and services.</rdfs:comment>
    <rdfs:domain rdf:resource="http://example.org/onto/class/google_cloud_run_domain_mapping"/>
    <rdfs:range rdf:resource="http://www.w3.org/2001/XMLSchema#string"/>
  </owl:DatatypeProperty>
  <owl:DatatypeProperty rdf:about="http://example.org/onto/prop/google_cloud_run_domain_mapping_generation">
    <rdfs:label>generation</rdfs:label>
    <rdfs:comment>A sequence number representing a specific generation of the desired state.</rdfs:comment>
    <rdfs:domain rdf:resource="http://example.org/onto/class/google_cloud_run_domain_mapping"/>
    <rdfs:range rdf:resource="http://www.w3.org/2001/XMLSchema#string"/>
  </owl:DatatypeProperty>
  <owl:DatatypeProperty rdf:about="http://example.org/onto/prop/google_cloud_run_domain_mapping_labels">
    <rdfs:label>labels</rdfs:label>
    <rdfs:comment>Map of string keys and values that can be used to organize and categorize
(scope and select) objects. May match selectors of replication controllers
and routes.
More info: https://kubernetes.io/docs/concepts/overview/working-with-objects/labels

**Note**: This field is non-authoritative, and will only manage the labels present in your configuration.
Please refer to the field 'effective_labels' for all of the labels present on the resource.</rdfs:comment>
    <rdfs:domain rdf:resource="http://example.org/onto/class/google_cloud_run_domain_mapping"/>
    <rdfs:range rdf:resource="http://www.w3.org/2001/XMLSchema#string"/>
  </owl:DatatypeProperty>
  <owl:DatatypeProperty rdf:about="http://example.org/onto/prop/google_cloud_run_domain_mapping_namespace">
    <rdfs:label>namespace</rdfs:label>
    <rdfs:comment>In Cloud Run the namespace must be equal to either the
project ID or project number.</rdfs:comment>
    <rdfs:domain rdf:resource="http://example.org/onto/class/google_cloud_run_domain_mapping"/>
    <rdfs:range rdf:resource="http://www.w3.org/2001/XMLSchema#string"/>
  </owl:DatatypeProperty>
  <owl:DatatypeProperty rdf:about="http://example.org/onto/prop/google_cloud_run_domain_mapping_resource_version">
    <rdfs:label>resource_version</rdfs:label>
    <rdfs:comment>An opaque value that represents the internal version of this object that
can be used by clients to determine when objects have changed. May be used
for optimistic concurrency, change detection, and the watch operation on a
resource or set of resources. They may only be valid for a
particular resource or set of resources.

More info:
https://git.k8s.io/community/contributors/devel/api-conventions.md#concurrency-control-and-consistency</rdfs:comment>
    <rdfs:domain rdf:resource="http://example.org/onto/class/google_cloud_run_domain_mapping"/>
    <rdfs:range rdf:resource="http://www.w3.org/2001/XMLSchema#string"/>
  </owl:DatatypeProperty>
  <owl:DatatypeProperty rdf:about="http://example.org/onto/prop/google_cloud_run_domain_mapping_self_link">
    <rdfs:label>self_link</rdfs:label>
    <rdfs:comment>SelfLink is a URL representing this object.</rdfs:comment>
    <rdfs:domain rdf:resource="http://example.org/onto/class/google_cloud_run_domain_mapping"/>
    <rdfs:range rdf:resource="http://www.w3.org/2001/XMLSchema#string"/>
  </owl:DatatypeProperty>
  <owl:DatatypeProperty rdf:about="http://example.org/onto/prop/google_cloud_run_domain_mapping_terraform_labels">
    <rdfs:label>terraform_labels</rdfs:label>
    <rdfs:comment>The combination of labels configured directly on the resource
 and default labels configured on the provider.</rdfs:comment>
    <rdfs:domain rdf:resource="http://example.org/onto/class/google_cloud_run_domain_mapping"/>
    <rdfs:range rdf:resource="http://www.w3.org/2001/XMLSchema#string"/>
  </owl:DatatypeProperty>
  <owl:DatatypeProperty rdf:about="http://example.org/onto/prop/google_cloud_run_domain_mapping_uid">
    <rdfs:label>uid</rdfs:label>
    <rdfs:comment>UID is a unique id generated by the server on successful creation of a resource and is not
allowed to change on PUT operations.

More info: https://kubernetes.io/docs/concepts/overview/working-with-objects/names#uids</rdfs:comment>
    <rdfs:domain rdf:resource="http://example.org/onto/class/google_cloud_run_domain_mapping"/>
    <rdfs:range rdf:resource="http://www.w3.org/2001/XMLSchema#string"/>
  </owl:DatatypeProperty>
  <owl:DatatypeProperty rdf:about="http://example.org/onto/prop/google_cloud_run_domain_mapping_certificate_mode">
    <rdfs:label>certificate_mode</rdfs:label>
    <rdfs:comment>The mode of the certificate. Default value: "AUTOMATIC" Possible values: ["NONE", "AUTOMATIC"]</rdfs:comment>
    <rdfs:domain rdf:resource="http://example.org/onto/class/google_cloud_run_domain_mapping"/>
    <rdfs:range rdf:resource="http://www.w3.org/2001/XMLSchema#string"/>
  </owl:DatatypeProperty>
  <owl:DatatypeProperty rdf:about="http://example.org/onto/prop/google_cloud_run_domain_mapping_force_override">
    <rdfs:label>force_override</rdfs:label>
    <rdfs:comment>If set, the mapping will override any mapping set before this spec was set.
It is recommended that the user leaves this empty to receive an error
warning about a potential conflict and only set it once the respective UI
has given such a warning.</rdfs:comment>
    <rdfs:domain rdf:resource="http://example.org/onto/class/google_cloud_run_domain_mapping"/>
    <rdfs:range rdf:resource="http://www.w3.org/2001/XMLSchema#string"/>
  </owl:DatatypeProperty>
  <owl:DatatypeProperty rdf:about="http://example.org/onto/prop/google_cloud_run_domain_mapping_route_name">
    <rdfs:label>route_name</rdfs:label>
    <rdfs:comment>The name of the Cloud Run Service that this DomainMapping applies to.
The route must exist.</rdfs:comment>
    <rdfs:domain rdf:resource="http://example.org/onto/class/google_cloud_run_domain_mapping"/>
    <rdfs:range rdf:resource="http://www.w3.org/2001/XMLSchema#string"/>
  </owl:DatatypeProperty>
  <owl:DatatypeProperty rdf:about="http://example.org/onto/prop/google_cloud_run_domain_mapping_create">
    <rdfs:label>create</rdfs:label>
    <rdfs:domain rdf:resource="http://example.org/onto/class/google_cloud_run_domain_mapping"/>
    <rdfs:range rdf:resource="http://www.w3.org/2001/XMLSchema#string"/>
  </owl:DatatypeProperty>
  <owl:DatatypeProperty rdf:about="http://example.org/onto/prop/google_cloud_run_domain_mapping_delete">
    <rdfs:label>delete</rdfs:label>
    <rdfs:domain rdf:resource="http://example.org/onto/class/google_cloud_run_domain_mapping"/>
    <rdfs:range rdf:resource="http://www.w3.org/2001/XMLSchema#string"/>
  </owl:DatatypeProperty>
</rdf:RDF>
