<?xml version="1.0" encoding="UTF-8"?>
<rdf:RDF
  xmlns:rdf="http://www.w3.org/1999/02/22-rdf-syntax-ns#"
  xmlns:rdfs="http://www.w3.org/2000/01/rdf-schema#"
  xmlns:owl="http://www.w3.org/2002/07/owl#"
  xmlns:xsd="http://www.w3.org/2001/XMLSchema#"
  xml:base="http://example.org/onto/">
  <owl:Class rdf:about="http://example.org/onto/class/google_discovery_engine_data_store">
    <rdfs:label>google_discovery_engine_data_store</rdfs:label>
    <rdfs:comment>#
#     ***     AUTO GENERATED CODE    ***    Type: MMv1     ***
#
# ----------------------------------------------------------------------------
#
#     This code is generated by Magic Modules using the following:
#
#     Configuration: https:#github.com/GoogleCloudPlatform/magic-modules/tree/main/mmv1/products/discoveryengine/DataStore.yaml
#     Template:      https:#github.com/GoogleCloudPlatform/magic-modules/tree/main/mmv1/templates/terraform/resource.html.markdown.tmpl
#
#     DO NOT EDIT this file directly. Any changes made to this file will be
#     overwritten during the next generation cycle.
#
# ----------------------------------------------------------------------------
subcategory: "Discovery Engine"
description: |-
  Data store is a collection of websites and documents used to find answers for
  end-user's questions in Discovery Engine (a.
---</rdfs:comment>
  </owl:Class>
  <owl:DatatypeProperty rdf:about="http://example.org/onto/prop/google_discovery_engine_data_store_content_config">
    <rdfs:label>content_config</rdfs:label>
    <rdfs:comment>The content config of the data store. Possible values: ["NO_CONTENT", "CONTENT_REQUIRED", "PUBLIC_WEBSITE"]</rdfs:comment>
    <rdfs:domain rdf:resource="http://example.org/onto/class/google_discovery_engine_data_store"/>
    <rdfs:range rdf:resource="http://www.w3.org/2001/XMLSchema#string"/>
  </owl:DatatypeProperty>
  <owl:DatatypeProperty rdf:about="http://example.org/onto/prop/google_discovery_engine_data_store_create_advanced_site_search">
    <rdfs:label>create_advanced_site_search</rdfs:label>
    <rdfs:comment>If true, an advanced data store for site search will be created. If the
data store is not configured as site search (GENERIC vertical and
PUBLIC_WEBSITE contentConfig), this flag will be ignored.</rdfs:comment>
    <rdfs:domain rdf:resource="http://example.org/onto/class/google_discovery_engine_data_store"/>
    <rdfs:range rdf:resource="http://www.w3.org/2001/XMLSchema#string"/>
  </owl:DatatypeProperty>
  <owl:DatatypeProperty rdf:about="http://example.org/onto/prop/google_discovery_engine_data_store_create_time">
    <rdfs:label>create_time</rdfs:label>
    <rdfs:comment>Timestamp when the DataStore was created.</rdfs:comment>
    <rdfs:domain rdf:resource="http://example.org/onto/class/google_discovery_engine_data_store"/>
    <rdfs:range rdf:resource="http://www.w3.org/2001/XMLSchema#string"/>
  </owl:DatatypeProperty>
  <owl:DatatypeProperty rdf:about="http://example.org/onto/prop/google_discovery_engine_data_store_data_store_id">
    <rdfs:label>data_store_id</rdfs:label>
    <rdfs:comment>The unique id of the data store.</rdfs:comment>
    <rdfs:domain rdf:resource="http://example.org/onto/class/google_discovery_engine_data_store"/>
    <rdfs:range rdf:resource="http://www.w3.org/2001/XMLSchema#string"/>
  </owl:DatatypeProperty>
  <owl:DatatypeProperty rdf:about="http://example.org/onto/prop/google_discovery_engine_data_store_default_schema_id">
    <rdfs:label>default_schema_id</rdfs:label>
    <rdfs:comment>The id of the default Schema associated with this data store.</rdfs:comment>
    <rdfs:domain rdf:resource="http://example.org/onto/class/google_discovery_engine_data_store"/>
    <rdfs:range rdf:resource="http://www.w3.org/2001/XMLSchema#string"/>
  </owl:DatatypeProperty>
  <owl:DatatypeProperty rdf:about="http://example.org/onto/prop/google_discovery_engine_data_store_display_name">
    <rdfs:label>display_name</rdfs:label>
    <rdfs:comment>The display name of the data store. This field must be a UTF-8 encoded
string with a length limit of 128 characters.</rdfs:comment>
    <rdfs:domain rdf:resource="http://example.org/onto/class/google_discovery_engine_data_store"/>
    <rdfs:range rdf:resource="http://www.w3.org/2001/XMLSchema#string"/>
  </owl:DatatypeProperty>
  <owl:DatatypeProperty rdf:about="http://example.org/onto/prop/google_discovery_engine_data_store_id">
    <rdfs:label>id</rdfs:label>
    <rdfs:domain rdf:resource="http://example.org/onto/class/google_discovery_engine_data_store"/>
    <rdfs:range rdf:resource="http://www.w3.org/2001/XMLSchema#string"/>
  </owl:DatatypeProperty>
  <owl:DatatypeProperty rdf:about="http://example.org/onto/prop/google_discovery_engine_data_store_industry_vertical">
    <rdfs:label>industry_vertical</rdfs:label>
    <rdfs:comment>The industry vertical that the data store registers. Possible values: ["GENERIC", "MEDIA", "HEALTHCARE_FHIR"]</rdfs:comment>
    <rdfs:domain rdf:resource="http://example.org/onto/class/google_discovery_engine_data_store"/>
    <rdfs:range rdf:resource="http://www.w3.org/2001/XMLSchema#string"/>
  </owl:DatatypeProperty>
  <owl:DatatypeProperty rdf:about="http://example.org/onto/prop/google_discovery_engine_data_store_kms_key_name">
    <rdfs:label>kms_key_name</rdfs:label>
    <rdfs:comment>KMS key resource name which will be used to encrypt resources:
'/{project}/locations/{location}/keyRings/{keyRing}/cryptoKeys/{keyId}'
The KMS key to be used to protect this DataStore at creation time. Must be
set for requests that need to comply with CMEK Org Policy protections.
If this field is set and processed successfully, the DataStore will be
protected by the KMS key, as indicated in the cmek_config field.</rdfs:comment>
    <rdfs:domain rdf:resource="http://example.org/onto/class/google_discovery_engine_data_store"/>
    <rdfs:range rdf:resource="http://www.w3.org/2001/XMLSchema#string"/>
  </owl:DatatypeProperty>
  <owl:DatatypeProperty rdf:about="http://example.org/onto/prop/google_discovery_engine_data_store_location">
    <rdfs:label>location</rdfs:label>
    <rdfs:comment>The geographic location where the data store should reside. The value can
only be one of "global", "us" and "eu".</rdfs:comment>
    <rdfs:domain rdf:resource="http://example.org/onto/class/google_discovery_engine_data_store"/>
    <rdfs:range rdf:resource="http://www.w3.org/2001/XMLSchema#string"/>
  </owl:DatatypeProperty>
  <owl:DatatypeProperty rdf:about="http://example.org/onto/prop/google_discovery_engine_data_store_name">
    <rdfs:label>name</rdfs:label>
    <rdfs:comment>The unique full resource name of the data store. Values are of the format
'projects/{project}/locations/{location}/collections/{collection_id}/dataStores/{data_store_id}'.
This field must be a UTF-8 encoded string with a length limit of 1024
characters.</rdfs:comment>
    <rdfs:domain rdf:resource="http://example.org/onto/class/google_discovery_engine_data_store"/>
    <rdfs:range rdf:resource="http://www.w3.org/2001/XMLSchema#string"/>
  </owl:DatatypeProperty>
  <owl:DatatypeProperty rdf:about="http://example.org/onto/prop/google_discovery_engine_data_store_project">
    <rdfs:label>project</rdfs:label>
    <rdfs:domain rdf:resource="http://example.org/onto/class/google_discovery_engine_data_store"/>
    <rdfs:range rdf:resource="http://www.w3.org/2001/XMLSchema#string"/>
  </owl:DatatypeProperty>
  <owl:DatatypeProperty rdf:about="http://example.org/onto/prop/google_discovery_engine_data_store_skip_default_schema_creation">
    <rdfs:label>skip_default_schema_creation</rdfs:label>
    <rdfs:comment>A boolean flag indicating whether to skip the default schema creation for
the data store. Only enable this flag if you are certain that the default
schema is incompatible with your use case.
If set to true, you must manually create a schema for the data store
before any documents can be ingested.
This flag cannot be specified if 'data_store.starting_schema' is
specified.</rdfs:comment>
    <rdfs:domain rdf:resource="http://example.org/onto/class/google_discovery_engine_data_store"/>
    <rdfs:range rdf:resource="http://www.w3.org/2001/XMLSchema#string"/>
  </owl:DatatypeProperty>
  <owl:DatatypeProperty rdf:about="http://example.org/onto/prop/google_discovery_engine_data_store_solution_types">
    <rdfs:label>solution_types</rdfs:label>
    <rdfs:comment>The solutions that the data store enrolls. Possible values: ["SOLUTION_TYPE_RECOMMENDATION", "SOLUTION_TYPE_SEARCH", "SOLUTION_TYPE_CHAT", "SOLUTION_TYPE_GENERATIVE_CHAT"]</rdfs:comment>
    <rdfs:domain rdf:resource="http://example.org/onto/class/google_discovery_engine_data_store"/>
    <rdfs:range rdf:resource="http://www.w3.org/2001/XMLSchema#string"/>
  </owl:DatatypeProperty>
  <owl:DatatypeProperty rdf:about="http://example.org/onto/prop/google_discovery_engine_data_store_disable_automatic_refresh">
    <rdfs:label>disable_automatic_refresh</rdfs:label>
    <rdfs:comment>If set true, automatic refresh is disabled for the DataStore.</rdfs:comment>
    <rdfs:domain rdf:resource="http://example.org/onto/class/google_discovery_engine_data_store"/>
    <rdfs:range rdf:resource="http://www.w3.org/2001/XMLSchema#string"/>
  </owl:DatatypeProperty>
  <owl:DatatypeProperty rdf:about="http://example.org/onto/prop/google_discovery_engine_data_store_disable_initial_index">
    <rdfs:label>disable_initial_index</rdfs:label>
    <rdfs:comment>If set true, initial indexing is disabled for the DataStore.</rdfs:comment>
    <rdfs:domain rdf:resource="http://example.org/onto/class/google_discovery_engine_data_store"/>
    <rdfs:range rdf:resource="http://www.w3.org/2001/XMLSchema#string"/>
  </owl:DatatypeProperty>
  <owl:DatatypeProperty rdf:about="http://example.org/onto/prop/google_discovery_engine_data_store_name">
    <rdfs:label>name</rdfs:label>
    <rdfs:comment>The full resource name of the Document Processing Config. Format:
'projects/{project}/locations/{location}/collections/{collection_id}/dataStores/{data_store_id}/documentProcessingConfig'.</rdfs:comment>
    <rdfs:domain rdf:resource="http://example.org/onto/class/google_discovery_engine_data_store"/>
    <rdfs:range rdf:resource="http://www.w3.org/2001/XMLSchema#string"/>
  </owl:DatatypeProperty>
  <owl:DatatypeProperty rdf:about="http://example.org/onto/prop/google_discovery_engine_data_store_chunk_size">
    <rdfs:label>chunk_size</rdfs:label>
    <rdfs:comment>The token size limit for each chunk.
Supported values: 100-500 (inclusive). Default value: 500.</rdfs:comment>
    <rdfs:domain rdf:resource="http://example.org/onto/class/google_discovery_engine_data_store"/>
    <rdfs:range rdf:resource="http://www.w3.org/2001/XMLSchema#string"/>
  </owl:DatatypeProperty>
  <owl:DatatypeProperty rdf:about="http://example.org/onto/prop/google_discovery_engine_data_store_include_ancestor_headings">
    <rdfs:label>include_ancestor_headings</rdfs:label>
    <rdfs:comment>Whether to include appending different levels of headings to chunks from the middle of the document to prevent context loss.
Default value: False.</rdfs:comment>
    <rdfs:domain rdf:resource="http://example.org/onto/class/google_discovery_engine_data_store"/>
    <rdfs:range rdf:resource="http://www.w3.org/2001/XMLSchema#string"/>
  </owl:DatatypeProperty>
  <owl:DatatypeProperty rdf:about="http://example.org/onto/prop/google_discovery_engine_data_store_enable_image_annotation">
    <rdfs:label>enable_image_annotation</rdfs:label>
    <rdfs:comment>If true, the LLM based annotation is added to the image during parsing.</rdfs:comment>
    <rdfs:domain rdf:resource="http://example.org/onto/class/google_discovery_engine_data_store"/>
    <rdfs:range rdf:resource="http://www.w3.org/2001/XMLSchema#string"/>
  </owl:DatatypeProperty>
  <owl:DatatypeProperty rdf:about="http://example.org/onto/prop/google_discovery_engine_data_store_enable_table_annotation">
    <rdfs:label>enable_table_annotation</rdfs:label>
    <rdfs:comment>If true, the LLM based annotation is added to the table during parsing.</rdfs:comment>
    <rdfs:domain rdf:resource="http://example.org/onto/class/google_discovery_engine_data_store"/>
    <rdfs:range rdf:resource="http://www.w3.org/2001/XMLSchema#string"/>
  </owl:DatatypeProperty>
  <owl:DatatypeProperty rdf:about="http://example.org/onto/prop/google_discovery_engine_data_store_exclude_html_classes">
    <rdfs:label>exclude_html_classes</rdfs:label>
    <rdfs:comment>List of HTML classes to exclude from the parsed content.</rdfs:comment>
    <rdfs:domain rdf:resource="http://example.org/onto/class/google_discovery_engine_data_store"/>
    <rdfs:range rdf:resource="http://www.w3.org/2001/XMLSchema#string"/>
  </owl:DatatypeProperty>
  <owl:DatatypeProperty rdf:about="http://example.org/onto/prop/google_discovery_engine_data_store_exclude_html_elements">
    <rdfs:label>exclude_html_elements</rdfs:label>
    <rdfs:comment>List of HTML elements to exclude from the parsed content.</rdfs:comment>
    <rdfs:domain rdf:resource="http://example.org/onto/class/google_discovery_engine_data_store"/>
    <rdfs:range rdf:resource="http://www.w3.org/2001/XMLSchema#string"/>
  </owl:DatatypeProperty>
  <owl:DatatypeProperty rdf:about="http://example.org/onto/prop/google_discovery_engine_data_store_exclude_html_ids">
    <rdfs:label>exclude_html_ids</rdfs:label>
    <rdfs:comment>List of HTML ids to exclude from the parsed content.</rdfs:comment>
    <rdfs:domain rdf:resource="http://example.org/onto/class/google_discovery_engine_data_store"/>
    <rdfs:range rdf:resource="http://www.w3.org/2001/XMLSchema#string"/>
  </owl:DatatypeProperty>
  <owl:DatatypeProperty rdf:about="http://example.org/onto/prop/google_discovery_engine_data_store_structured_content_types">
    <rdfs:label>structured_content_types</rdfs:label>
    <rdfs:comment>Contains the required structure types to extract from the document. Supported values: 'shareholder-structure'.</rdfs:comment>
    <rdfs:domain rdf:resource="http://example.org/onto/class/google_discovery_engine_data_store"/>
    <rdfs:range rdf:resource="http://www.w3.org/2001/XMLSchema#string"/>
  </owl:DatatypeProperty>
  <owl:DatatypeProperty rdf:about="http://example.org/onto/prop/google_discovery_engine_data_store_use_native_text">
    <rdfs:label>use_native_text</rdfs:label>
    <rdfs:comment>If true, will use native text instead of OCR text on pages containing native text.</rdfs:comment>
    <rdfs:domain rdf:resource="http://example.org/onto/class/google_discovery_engine_data_store"/>
    <rdfs:range rdf:resource="http://www.w3.org/2001/XMLSchema#string"/>
  </owl:DatatypeProperty>
  <owl:DatatypeProperty rdf:about="http://example.org/onto/prop/google_discovery_engine_data_store_file_type">
    <rdfs:label>file_type</rdfs:label>
    <rdfs:domain rdf:resource="http://example.org/onto/class/google_discovery_engine_data_store"/>
    <rdfs:range rdf:resource="http://www.w3.org/2001/XMLSchema#string"/>
  </owl:DatatypeProperty>
  <owl:DatatypeProperty rdf:about="http://example.org/onto/prop/google_discovery_engine_data_store_enable_image_annotation">
    <rdfs:label>enable_image_annotation</rdfs:label>
    <rdfs:comment>If true, the LLM based annotation is added to the image during parsing.</rdfs:comment>
    <rdfs:domain rdf:resource="http://example.org/onto/class/google_discovery_engine_data_store"/>
    <rdfs:range rdf:resource="http://www.w3.org/2001/XMLSchema#string"/>
  </owl:DatatypeProperty>
  <owl:DatatypeProperty rdf:about="http://example.org/onto/prop/google_discovery_engine_data_store_enable_table_annotation">
    <rdfs:label>enable_table_annotation</rdfs:label>
    <rdfs:comment>If true, the LLM based annotation is added to the table during parsing.</rdfs:comment>
    <rdfs:domain rdf:resource="http://example.org/onto/class/google_discovery_engine_data_store"/>
    <rdfs:range rdf:resource="http://www.w3.org/2001/XMLSchema#string"/>
  </owl:DatatypeProperty>
  <owl:DatatypeProperty rdf:about="http://example.org/onto/prop/google_discovery_engine_data_store_exclude_html_classes">
    <rdfs:label>exclude_html_classes</rdfs:label>
    <rdfs:comment>List of HTML classes to exclude from the parsed content.</rdfs:comment>
    <rdfs:domain rdf:resource="http://example.org/onto/class/google_discovery_engine_data_store"/>
    <rdfs:range rdf:resource="http://www.w3.org/2001/XMLSchema#string"/>
  </owl:DatatypeProperty>
  <owl:DatatypeProperty rdf:about="http://example.org/onto/prop/google_discovery_engine_data_store_exclude_html_elements">
    <rdfs:label>exclude_html_elements</rdfs:label>
    <rdfs:comment>List of HTML elements to exclude from the parsed content.</rdfs:comment>
    <rdfs:domain rdf:resource="http://example.org/onto/class/google_discovery_engine_data_store"/>
    <rdfs:range rdf:resource="http://www.w3.org/2001/XMLSchema#string"/>
  </owl:DatatypeProperty>
  <owl:DatatypeProperty rdf:about="http://example.org/onto/prop/google_discovery_engine_data_store_exclude_html_ids">
    <rdfs:label>exclude_html_ids</rdfs:label>
    <rdfs:comment>List of HTML ids to exclude from the parsed content.</rdfs:comment>
    <rdfs:domain rdf:resource="http://example.org/onto/class/google_discovery_engine_data_store"/>
    <rdfs:range rdf:resource="http://www.w3.org/2001/XMLSchema#string"/>
  </owl:DatatypeProperty>
  <owl:DatatypeProperty rdf:about="http://example.org/onto/prop/google_discovery_engine_data_store_structured_content_types">
    <rdfs:label>structured_content_types</rdfs:label>
    <rdfs:comment>Contains the required structure types to extract from the document. Supported values: 'shareholder-structure'.</rdfs:comment>
    <rdfs:domain rdf:resource="http://example.org/onto/class/google_discovery_engine_data_store"/>
    <rdfs:range rdf:resource="http://www.w3.org/2001/XMLSchema#string"/>
  </owl:DatatypeProperty>
  <owl:DatatypeProperty rdf:about="http://example.org/onto/prop/google_discovery_engine_data_store_use_native_text">
    <rdfs:label>use_native_text</rdfs:label>
    <rdfs:comment>If true, will use native text instead of OCR text on pages containing native text.</rdfs:comment>
    <rdfs:domain rdf:resource="http://example.org/onto/class/google_discovery_engine_data_store"/>
    <rdfs:range rdf:resource="http://www.w3.org/2001/XMLSchema#string"/>
  </owl:DatatypeProperty>
  <owl:DatatypeProperty rdf:about="http://example.org/onto/prop/google_discovery_engine_data_store_create">
    <rdfs:label>create</rdfs:label>
    <rdfs:domain rdf:resource="http://example.org/onto/class/google_discovery_engine_data_store"/>
    <rdfs:range rdf:resource="http://www.w3.org/2001/XMLSchema#string"/>
  </owl:DatatypeProperty>
  <owl:DatatypeProperty rdf:about="http://example.org/onto/prop/google_discovery_engine_data_store_delete">
    <rdfs:label>delete</rdfs:label>
    <rdfs:domain rdf:resource="http://example.org/onto/class/google_discovery_engine_data_store"/>
    <rdfs:range rdf:resource="http://www.w3.org/2001/XMLSchema#string"/>
  </owl:DatatypeProperty>
  <owl:DatatypeProperty rdf:about="http://example.org/onto/prop/google_discovery_engine_data_store_update">
    <rdfs:label>update</rdfs:label>
    <rdfs:domain rdf:resource="http://example.org/onto/class/google_discovery_engine_data_store"/>
    <rdfs:range rdf:resource="http://www.w3.org/2001/XMLSchema#string"/>
  </owl:DatatypeProperty>
</rdf:RDF>
