<?xml version="1.0" encoding="UTF-8"?>
<rdf:RDF
  xmlns:rdf="http://www.w3.org/1999/02/22-rdf-syntax-ns#"
  xmlns:rdfs="http://www.w3.org/2000/01/rdf-schema#"
  xmlns:owl="http://www.w3.org/2002/07/owl#"
  xmlns:xsd="http://www.w3.org/2001/XMLSchema#"
  xml:base="http://example.org/onto/">
  <owl:Class rdf:about="http://example.org/onto/class/google_storage_insights_dataset_config">
    <rdfs:label>google_storage_insights_dataset_config</rdfs:label>
    <rdfs:comment>#
#     ***     AUTO GENERATED CODE    ***    Type: MMv1     ***
#
# ----------------------------------------------------------------------------
#
#     This code is generated by Magic Modules using the following:
#
#     Configuration: https:#github.com/GoogleCloudPlatform/magic-modules/tree/main/mmv1/products/storageinsights/DatasetConfig.yaml
#     Template:      https:#github.com/GoogleCloudPlatform/magic-modules/tree/main/mmv1/templates/terraform/resource.html.markdown.tmpl
#
#     DO NOT EDIT this file directly. Any changes made to this file will be
#     overwritten during the next generation cycle.
#
# ----------------------------------------------------------------------------
subcategory: "Cloud Storage Insights"
description: |-
  Represents a Storage Insights DatasetConfig.
---</rdfs:comment>
  </owl:Class>
  <owl:DatatypeProperty rdf:about="http://example.org/onto/prop/google_storage_insights_dataset_config_create_time">
    <rdfs:label>create_time</rdfs:label>
    <rdfs:comment>The UTC time at which the DatasetConfig was created. This is auto-populated.</rdfs:comment>
    <rdfs:domain rdf:resource="http://example.org/onto/class/google_storage_insights_dataset_config"/>
    <rdfs:range rdf:resource="http://www.w3.org/2001/XMLSchema#string"/>
  </owl:DatatypeProperty>
  <owl:DatatypeProperty rdf:about="http://example.org/onto/prop/google_storage_insights_dataset_config_dataset_config_id">
    <rdfs:label>dataset_config_id</rdfs:label>
    <rdfs:comment>The user-defined ID of the DatasetConfig</rdfs:comment>
    <rdfs:domain rdf:resource="http://example.org/onto/class/google_storage_insights_dataset_config"/>
    <rdfs:range rdf:resource="http://www.w3.org/2001/XMLSchema#string"/>
  </owl:DatatypeProperty>
  <owl:DatatypeProperty rdf:about="http://example.org/onto/prop/google_storage_insights_dataset_config_dataset_config_state">
    <rdfs:label>dataset_config_state</rdfs:label>
    <rdfs:comment>State of the DatasetConfig.</rdfs:comment>
    <rdfs:domain rdf:resource="http://example.org/onto/class/google_storage_insights_dataset_config"/>
    <rdfs:range rdf:resource="http://www.w3.org/2001/XMLSchema#string"/>
  </owl:DatatypeProperty>
  <owl:DatatypeProperty rdf:about="http://example.org/onto/prop/google_storage_insights_dataset_config_description">
    <rdfs:label>description</rdfs:label>
    <rdfs:comment>An optional user-provided description for the dataset configuration with a maximum length of 256 characters.</rdfs:comment>
    <rdfs:domain rdf:resource="http://example.org/onto/class/google_storage_insights_dataset_config"/>
    <rdfs:range rdf:resource="http://www.w3.org/2001/XMLSchema#string"/>
  </owl:DatatypeProperty>
  <owl:DatatypeProperty rdf:about="http://example.org/onto/prop/google_storage_insights_dataset_config_id">
    <rdfs:label>id</rdfs:label>
    <rdfs:domain rdf:resource="http://example.org/onto/class/google_storage_insights_dataset_config"/>
    <rdfs:range rdf:resource="http://www.w3.org/2001/XMLSchema#string"/>
  </owl:DatatypeProperty>
  <owl:DatatypeProperty rdf:about="http://example.org/onto/prop/google_storage_insights_dataset_config_include_newly_created_buckets">
    <rdfs:label>include_newly_created_buckets</rdfs:label>
    <rdfs:comment>If set to true, the request includes all the newly created buckets in the dataset that meet the inclusion and exclusion rules.</rdfs:comment>
    <rdfs:domain rdf:resource="http://example.org/onto/class/google_storage_insights_dataset_config"/>
    <rdfs:range rdf:resource="http://www.w3.org/2001/XMLSchema#string"/>
  </owl:DatatypeProperty>
  <owl:DatatypeProperty rdf:about="http://example.org/onto/prop/google_storage_insights_dataset_config_link">
    <rdfs:label>link</rdfs:label>
    <rdfs:comment>Details of the linked DatasetConfig.</rdfs:comment>
    <rdfs:domain rdf:resource="http://example.org/onto/class/google_storage_insights_dataset_config"/>
    <rdfs:range rdf:resource="http://www.w3.org/2001/XMLSchema#string"/>
  </owl:DatatypeProperty>
  <owl:DatatypeProperty rdf:about="http://example.org/onto/prop/google_storage_insights_dataset_config_link_dataset">
    <rdfs:label>link_dataset</rdfs:label>
    <rdfs:comment>A boolean terraform only flag to link/unlink dataset.

Setting this field to true while creation will automatically link the created dataset as an additional functionality.
-> **Note** A dataset config resource can only be destroyed once it is unlinked,
so users must set this field to false to unlink the dataset and destroy the dataset config resource.</rdfs:comment>
    <rdfs:domain rdf:resource="http://example.org/onto/class/google_storage_insights_dataset_config"/>
    <rdfs:range rdf:resource="http://www.w3.org/2001/XMLSchema#string"/>
  </owl:DatatypeProperty>
  <owl:DatatypeProperty rdf:about="http://example.org/onto/prop/google_storage_insights_dataset_config_location">
    <rdfs:label>location</rdfs:label>
    <rdfs:comment>The location of the DatasetConfig.</rdfs:comment>
    <rdfs:domain rdf:resource="http://example.org/onto/class/google_storage_insights_dataset_config"/>
    <rdfs:range rdf:resource="http://www.w3.org/2001/XMLSchema#string"/>
  </owl:DatatypeProperty>
  <owl:DatatypeProperty rdf:about="http://example.org/onto/prop/google_storage_insights_dataset_config_name">
    <rdfs:label>name</rdfs:label>
    <rdfs:comment>The full canonical resource name of the DatasetConfig (e.g., projects/P/locations/L/datasetConfigs/ID).</rdfs:comment>
    <rdfs:domain rdf:resource="http://example.org/onto/class/google_storage_insights_dataset_config"/>
    <rdfs:range rdf:resource="http://www.w3.org/2001/XMLSchema#string"/>
  </owl:DatatypeProperty>
  <owl:DatatypeProperty rdf:about="http://example.org/onto/prop/google_storage_insights_dataset_config_organization_number">
    <rdfs:label>organization_number</rdfs:label>
    <rdfs:comment>Organization resource ID that the source projects should belong to.
Projects that do not belong to the provided organization are not considered when creating the dataset.</rdfs:comment>
    <rdfs:domain rdf:resource="http://example.org/onto/class/google_storage_insights_dataset_config"/>
    <rdfs:range rdf:resource="http://www.w3.org/2001/XMLSchema#string"/>
  </owl:DatatypeProperty>
  <owl:DatatypeProperty rdf:about="http://example.org/onto/prop/google_storage_insights_dataset_config_organization_scope">
    <rdfs:label>organization_scope</rdfs:label>
    <rdfs:comment>Defines the options for providing a source organization for the DatasetConfig.</rdfs:comment>
    <rdfs:domain rdf:resource="http://example.org/onto/class/google_storage_insights_dataset_config"/>
    <rdfs:range rdf:resource="http://www.w3.org/2001/XMLSchema#string"/>
  </owl:DatatypeProperty>
  <owl:DatatypeProperty rdf:about="http://example.org/onto/prop/google_storage_insights_dataset_config_project">
    <rdfs:label>project</rdfs:label>
    <rdfs:domain rdf:resource="http://example.org/onto/class/google_storage_insights_dataset_config"/>
    <rdfs:range rdf:resource="http://www.w3.org/2001/XMLSchema#string"/>
  </owl:DatatypeProperty>
  <owl:DatatypeProperty rdf:about="http://example.org/onto/prop/google_storage_insights_dataset_config_retention_period_days">
    <rdfs:label>retention_period_days</rdfs:label>
    <rdfs:comment>Number of days of history that must be retained.</rdfs:comment>
    <rdfs:domain rdf:resource="http://example.org/onto/class/google_storage_insights_dataset_config"/>
    <rdfs:range rdf:resource="http://www.w3.org/2001/XMLSchema#string"/>
  </owl:DatatypeProperty>
  <owl:DatatypeProperty rdf:about="http://example.org/onto/prop/google_storage_insights_dataset_config_uid">
    <rdfs:label>uid</rdfs:label>
    <rdfs:comment>System generated unique identifier for the resource.</rdfs:comment>
    <rdfs:domain rdf:resource="http://example.org/onto/class/google_storage_insights_dataset_config"/>
    <rdfs:range rdf:resource="http://www.w3.org/2001/XMLSchema#string"/>
  </owl:DatatypeProperty>
  <owl:DatatypeProperty rdf:about="http://example.org/onto/prop/google_storage_insights_dataset_config_update_time">
    <rdfs:label>update_time</rdfs:label>
    <rdfs:comment>The UTC time at which the DatasetConfig was updated. This is auto-populated.</rdfs:comment>
    <rdfs:domain rdf:resource="http://example.org/onto/class/google_storage_insights_dataset_config"/>
    <rdfs:range rdf:resource="http://www.w3.org/2001/XMLSchema#string"/>
  </owl:DatatypeProperty>
  <owl:DatatypeProperty rdf:about="http://example.org/onto/prop/google_storage_insights_dataset_config_bucket_name">
    <rdfs:label>bucket_name</rdfs:label>
    <rdfs:comment>The list of cloud storage bucket names to exclude in the DatasetConfig.
Exactly one of the bucket_name and bucket_prefix_regex should be specified.</rdfs:comment>
    <rdfs:domain rdf:resource="http://example.org/onto/class/google_storage_insights_dataset_config"/>
    <rdfs:range rdf:resource="http://www.w3.org/2001/XMLSchema#string"/>
  </owl:DatatypeProperty>
  <owl:DatatypeProperty rdf:about="http://example.org/onto/prop/google_storage_insights_dataset_config_bucket_prefix_regex">
    <rdfs:label>bucket_prefix_regex</rdfs:label>
    <rdfs:comment>The list of regex patterns for bucket names matching the regex.
Regex should follow the syntax specified in google/re2 on GitHub.
Exactly one of the bucket_name and bucket_prefix_regex should be specified.</rdfs:comment>
    <rdfs:domain rdf:resource="http://example.org/onto/class/google_storage_insights_dataset_config"/>
    <rdfs:range rdf:resource="http://www.w3.org/2001/XMLSchema#string"/>
  </owl:DatatypeProperty>
  <owl:DatatypeProperty rdf:about="http://example.org/onto/prop/google_storage_insights_dataset_config_locations">
    <rdfs:label>locations</rdfs:label>
    <rdfs:comment>The list of cloud storage locations to exclude in the DatasetConfig.</rdfs:comment>
    <rdfs:domain rdf:resource="http://example.org/onto/class/google_storage_insights_dataset_config"/>
    <rdfs:range rdf:resource="http://www.w3.org/2001/XMLSchema#string"/>
  </owl:DatatypeProperty>
  <owl:DatatypeProperty rdf:about="http://example.org/onto/prop/google_storage_insights_dataset_config_name">
    <rdfs:label>name</rdfs:label>
    <rdfs:comment>Name of the identity.</rdfs:comment>
    <rdfs:domain rdf:resource="http://example.org/onto/class/google_storage_insights_dataset_config"/>
    <rdfs:range rdf:resource="http://www.w3.org/2001/XMLSchema#string"/>
  </owl:DatatypeProperty>
  <owl:DatatypeProperty rdf:about="http://example.org/onto/prop/google_storage_insights_dataset_config_type">
    <rdfs:label>type</rdfs:label>
    <rdfs:comment>Type of identity to use for the DatasetConfig. Possible values: ["IDENTITY_TYPE_PER_CONFIG", "IDENTITY_TYPE_PER_PROJECT"]</rdfs:comment>
    <rdfs:domain rdf:resource="http://example.org/onto/class/google_storage_insights_dataset_config"/>
    <rdfs:range rdf:resource="http://www.w3.org/2001/XMLSchema#string"/>
  </owl:DatatypeProperty>
  <owl:DatatypeProperty rdf:about="http://example.org/onto/prop/google_storage_insights_dataset_config_bucket_name">
    <rdfs:label>bucket_name</rdfs:label>
    <rdfs:comment>The list of cloud storage bucket names to include in the DatasetConfig.
Exactly one of the bucket_name and bucket_prefix_regex should be specified.</rdfs:comment>
    <rdfs:domain rdf:resource="http://example.org/onto/class/google_storage_insights_dataset_config"/>
    <rdfs:range rdf:resource="http://www.w3.org/2001/XMLSchema#string"/>
  </owl:DatatypeProperty>
  <owl:DatatypeProperty rdf:about="http://example.org/onto/prop/google_storage_insights_dataset_config_bucket_prefix_regex">
    <rdfs:label>bucket_prefix_regex</rdfs:label>
    <rdfs:comment>The list of regex patterns for bucket names matching the regex.
Regex should follow the syntax specified in google/re2 on GitHub.
Exactly one of the bucket_name and bucket_prefix_regex should be specified.</rdfs:comment>
    <rdfs:domain rdf:resource="http://example.org/onto/class/google_storage_insights_dataset_config"/>
    <rdfs:range rdf:resource="http://www.w3.org/2001/XMLSchema#string"/>
  </owl:DatatypeProperty>
  <owl:DatatypeProperty rdf:about="http://example.org/onto/prop/google_storage_insights_dataset_config_locations">
    <rdfs:label>locations</rdfs:label>
    <rdfs:comment>The list of cloud storage locations to include in the DatasetConfig.</rdfs:comment>
    <rdfs:domain rdf:resource="http://example.org/onto/class/google_storage_insights_dataset_config"/>
    <rdfs:range rdf:resource="http://www.w3.org/2001/XMLSchema#string"/>
  </owl:DatatypeProperty>
  <owl:DatatypeProperty rdf:about="http://example.org/onto/prop/google_storage_insights_dataset_config_folder_numbers">
    <rdfs:label>folder_numbers</rdfs:label>
    <rdfs:comment>The list of folder numbers to include in the DatasetConfig.</rdfs:comment>
    <rdfs:domain rdf:resource="http://example.org/onto/class/google_storage_insights_dataset_config"/>
    <rdfs:range rdf:resource="http://www.w3.org/2001/XMLSchema#string"/>
  </owl:DatatypeProperty>
  <owl:DatatypeProperty rdf:about="http://example.org/onto/prop/google_storage_insights_dataset_config_project_numbers">
    <rdfs:label>project_numbers</rdfs:label>
    <rdfs:comment>The list of project numbers to include in the DatasetConfig.</rdfs:comment>
    <rdfs:domain rdf:resource="http://example.org/onto/class/google_storage_insights_dataset_config"/>
    <rdfs:range rdf:resource="http://www.w3.org/2001/XMLSchema#string"/>
  </owl:DatatypeProperty>
  <owl:DatatypeProperty rdf:about="http://example.org/onto/prop/google_storage_insights_dataset_config_create">
    <rdfs:label>create</rdfs:label>
    <rdfs:domain rdf:resource="http://example.org/onto/class/google_storage_insights_dataset_config"/>
    <rdfs:range rdf:resource="http://www.w3.org/2001/XMLSchema#string"/>
  </owl:DatatypeProperty>
  <owl:DatatypeProperty rdf:about="http://example.org/onto/prop/google_storage_insights_dataset_config_delete">
    <rdfs:label>delete</rdfs:label>
    <rdfs:domain rdf:resource="http://example.org/onto/class/google_storage_insights_dataset_config"/>
    <rdfs:range rdf:resource="http://www.w3.org/2001/XMLSchema#string"/>
  </owl:DatatypeProperty>
  <owl:DatatypeProperty rdf:about="http://example.org/onto/prop/google_storage_insights_dataset_config_update">
    <rdfs:label>update</rdfs:label>
    <rdfs:domain rdf:resource="http://example.org/onto/class/google_storage_insights_dataset_config"/>
    <rdfs:range rdf:resource="http://www.w3.org/2001/XMLSchema#string"/>
  </owl:DatatypeProperty>
</rdf:RDF>
