<?xml version="1.0" encoding="UTF-8"?>
<rdf:RDF
  xmlns:rdf="http://www.w3.org/1999/02/22-rdf-syntax-ns#"
  xmlns:rdfs="http://www.w3.org/2000/01/rdf-schema#"
  xmlns:owl="http://www.w3.org/2002/07/owl#"
  xmlns:xsd="http://www.w3.org/2001/XMLSchema#"
  xml:base="http://example.org/onto/">
  <owl:Class rdf:about="http://example.org/onto/class/google_database_migration_service_connection_profile">
    <rdfs:label>google_database_migration_service_connection_profile</rdfs:label>
    <rdfs:comment>#
#     ***     AUTO GENERATED CODE    ***    Type: MMv1     ***
#
# ----------------------------------------------------------------------------
#
#     This code is generated by Magic Modules using the following:
#
#     Configuration: https:#github.com/GoogleCloudPlatform/magic-modules/tree/main/mmv1/products/databasemigrationservice/ConnectionProfile.yaml
#     Template:      https:#github.com/GoogleCloudPlatform/magic-modules/tree/main/mmv1/templates/terraform/resource.html.markdown.tmpl
#
#     DO NOT EDIT this file directly. Any changes made to this file will be
#     overwritten during the next generation cycle.
#
# ----------------------------------------------------------------------------
subcategory: "DatabaseMigrationService"
description: |-
  A connection profile definition.
---</rdfs:comment>
  </owl:Class>
  <owl:DatatypeProperty rdf:about="http://example.org/onto/prop/google_database_migration_service_connection_profile_connection_profile_id">
    <rdfs:label>connection_profile_id</rdfs:label>
    <rdfs:comment>The ID of the connection profile.</rdfs:comment>
    <rdfs:domain rdf:resource="http://example.org/onto/class/google_database_migration_service_connection_profile"/>
    <rdfs:range rdf:resource="http://www.w3.org/2001/XMLSchema#string"/>
  </owl:DatatypeProperty>
  <owl:DatatypeProperty rdf:about="http://example.org/onto/prop/google_database_migration_service_connection_profile_create_time">
    <rdfs:label>create_time</rdfs:label>
    <rdfs:comment>Output only. The timestamp when the resource was created. A timestamp in RFC3339 UTC 'Zulu' format, accurate to nanoseconds. Example: '2014-10-02T15:01:23.045123456Z'.</rdfs:comment>
    <rdfs:domain rdf:resource="http://example.org/onto/class/google_database_migration_service_connection_profile"/>
    <rdfs:range rdf:resource="http://www.w3.org/2001/XMLSchema#string"/>
  </owl:DatatypeProperty>
  <owl:DatatypeProperty rdf:about="http://example.org/onto/prop/google_database_migration_service_connection_profile_dbprovider">
    <rdfs:label>dbprovider</rdfs:label>
    <rdfs:comment>The database provider.</rdfs:comment>
    <rdfs:domain rdf:resource="http://example.org/onto/class/google_database_migration_service_connection_profile"/>
    <rdfs:range rdf:resource="http://www.w3.org/2001/XMLSchema#string"/>
  </owl:DatatypeProperty>
  <owl:DatatypeProperty rdf:about="http://example.org/onto/prop/google_database_migration_service_connection_profile_display_name">
    <rdfs:label>display_name</rdfs:label>
    <rdfs:comment>The connection profile display name.</rdfs:comment>
    <rdfs:domain rdf:resource="http://example.org/onto/class/google_database_migration_service_connection_profile"/>
    <rdfs:range rdf:resource="http://www.w3.org/2001/XMLSchema#string"/>
  </owl:DatatypeProperty>
  <owl:DatatypeProperty rdf:about="http://example.org/onto/prop/google_database_migration_service_connection_profile_effective_labels">
    <rdfs:label>effective_labels</rdfs:label>
    <rdfs:comment>All of labels (key/value pairs) present on the resource in GCP, including the labels configured through Terraform, other clients and services.</rdfs:comment>
    <rdfs:domain rdf:resource="http://example.org/onto/class/google_database_migration_service_connection_profile"/>
    <rdfs:range rdf:resource="http://www.w3.org/2001/XMLSchema#string"/>
  </owl:DatatypeProperty>
  <owl:DatatypeProperty rdf:about="http://example.org/onto/prop/google_database_migration_service_connection_profile_error">
    <rdfs:label>error</rdfs:label>
    <rdfs:comment>Output only. The error details in case of state FAILED.</rdfs:comment>
    <rdfs:domain rdf:resource="http://example.org/onto/class/google_database_migration_service_connection_profile"/>
    <rdfs:range rdf:resource="http://www.w3.org/2001/XMLSchema#string"/>
  </owl:DatatypeProperty>
  <owl:DatatypeProperty rdf:about="http://example.org/onto/prop/google_database_migration_service_connection_profile_id">
    <rdfs:label>id</rdfs:label>
    <rdfs:domain rdf:resource="http://example.org/onto/class/google_database_migration_service_connection_profile"/>
    <rdfs:range rdf:resource="http://www.w3.org/2001/XMLSchema#string"/>
  </owl:DatatypeProperty>
  <owl:DatatypeProperty rdf:about="http://example.org/onto/prop/google_database_migration_service_connection_profile_labels">
    <rdfs:label>labels</rdfs:label>
    <rdfs:comment>The resource labels for connection profile to use to annotate any related underlying resources such as Compute Engine VMs.


**Note**: This field is non-authoritative, and will only manage the labels present in your configuration.
Please refer to the field 'effective_labels' for all of the labels present on the resource.</rdfs:comment>
    <rdfs:domain rdf:resource="http://example.org/onto/class/google_database_migration_service_connection_profile"/>
    <rdfs:range rdf:resource="http://www.w3.org/2001/XMLSchema#string"/>
  </owl:DatatypeProperty>
  <owl:DatatypeProperty rdf:about="http://example.org/onto/prop/google_database_migration_service_connection_profile_location">
    <rdfs:label>location</rdfs:label>
    <rdfs:comment>The location where the connection profile should reside.</rdfs:comment>
    <rdfs:domain rdf:resource="http://example.org/onto/class/google_database_migration_service_connection_profile"/>
    <rdfs:range rdf:resource="http://www.w3.org/2001/XMLSchema#string"/>
  </owl:DatatypeProperty>
  <owl:DatatypeProperty rdf:about="http://example.org/onto/prop/google_database_migration_service_connection_profile_name">
    <rdfs:label>name</rdfs:label>
    <rdfs:comment>The name of this connection profile resource in the form of projects/{project}/locations/{location}/connectionProfiles/{connectionProfile}.</rdfs:comment>
    <rdfs:domain rdf:resource="http://example.org/onto/class/google_database_migration_service_connection_profile"/>
    <rdfs:range rdf:resource="http://www.w3.org/2001/XMLSchema#string"/>
  </owl:DatatypeProperty>
  <owl:DatatypeProperty rdf:about="http://example.org/onto/prop/google_database_migration_service_connection_profile_project">
    <rdfs:label>project</rdfs:label>
    <rdfs:domain rdf:resource="http://example.org/onto/class/google_database_migration_service_connection_profile"/>
    <rdfs:range rdf:resource="http://www.w3.org/2001/XMLSchema#string"/>
  </owl:DatatypeProperty>
  <owl:DatatypeProperty rdf:about="http://example.org/onto/prop/google_database_migration_service_connection_profile_state">
    <rdfs:label>state</rdfs:label>
    <rdfs:comment>The current connection profile state.</rdfs:comment>
    <rdfs:domain rdf:resource="http://example.org/onto/class/google_database_migration_service_connection_profile"/>
    <rdfs:range rdf:resource="http://www.w3.org/2001/XMLSchema#string"/>
  </owl:DatatypeProperty>
  <owl:DatatypeProperty rdf:about="http://example.org/onto/prop/google_database_migration_service_connection_profile_terraform_labels">
    <rdfs:label>terraform_labels</rdfs:label>
    <rdfs:comment>The combination of labels configured directly on the resource
 and default labels configured on the provider.</rdfs:comment>
    <rdfs:domain rdf:resource="http://example.org/onto/class/google_database_migration_service_connection_profile"/>
    <rdfs:range rdf:resource="http://www.w3.org/2001/XMLSchema#string"/>
  </owl:DatatypeProperty>
  <owl:DatatypeProperty rdf:about="http://example.org/onto/prop/google_database_migration_service_connection_profile_cluster_id">
    <rdfs:label>cluster_id</rdfs:label>
    <rdfs:comment>Required. The AlloyDB cluster ID that this connection profile is associated with.</rdfs:comment>
    <rdfs:domain rdf:resource="http://example.org/onto/class/google_database_migration_service_connection_profile"/>
    <rdfs:range rdf:resource="http://www.w3.org/2001/XMLSchema#string"/>
  </owl:DatatypeProperty>
  <owl:DatatypeProperty rdf:about="http://example.org/onto/prop/google_database_migration_service_connection_profile_labels">
    <rdfs:label>labels</rdfs:label>
    <rdfs:comment>Labels for the AlloyDB cluster created by DMS.</rdfs:comment>
    <rdfs:domain rdf:resource="http://example.org/onto/class/google_database_migration_service_connection_profile"/>
    <rdfs:range rdf:resource="http://www.w3.org/2001/XMLSchema#string"/>
  </owl:DatatypeProperty>
  <owl:DatatypeProperty rdf:about="http://example.org/onto/prop/google_database_migration_service_connection_profile_vpc_network">
    <rdfs:label>vpc_network</rdfs:label>
    <rdfs:comment>Required. The resource link for the VPC network in which cluster resources are created and from which they are accessible via Private IP. The network must belong to the same project as the cluster.
It is specified in the form: 'projects/{project_number}/global/networks/{network_id}'. This is required to create a cluster.</rdfs:comment>
    <rdfs:domain rdf:resource="http://example.org/onto/class/google_database_migration_service_connection_profile"/>
    <rdfs:range rdf:resource="http://www.w3.org/2001/XMLSchema#string"/>
  </owl:DatatypeProperty>
  <owl:DatatypeProperty rdf:about="http://example.org/onto/prop/google_database_migration_service_connection_profile_password">
    <rdfs:label>password</rdfs:label>
    <rdfs:comment>The initial password for the user.</rdfs:comment>
    <rdfs:domain rdf:resource="http://example.org/onto/class/google_database_migration_service_connection_profile"/>
    <rdfs:range rdf:resource="http://www.w3.org/2001/XMLSchema#string"/>
  </owl:DatatypeProperty>
  <owl:DatatypeProperty rdf:about="http://example.org/onto/prop/google_database_migration_service_connection_profile_password_set">
    <rdfs:label>password_set</rdfs:label>
    <rdfs:comment>Output only. Indicates if the initialUser.password field has been set.</rdfs:comment>
    <rdfs:domain rdf:resource="http://example.org/onto/class/google_database_migration_service_connection_profile"/>
    <rdfs:range rdf:resource="http://www.w3.org/2001/XMLSchema#string"/>
  </owl:DatatypeProperty>
  <owl:DatatypeProperty rdf:about="http://example.org/onto/prop/google_database_migration_service_connection_profile_user">
    <rdfs:label>user</rdfs:label>
    <rdfs:comment>The database username.</rdfs:comment>
    <rdfs:domain rdf:resource="http://example.org/onto/class/google_database_migration_service_connection_profile"/>
    <rdfs:range rdf:resource="http://www.w3.org/2001/XMLSchema#string"/>
  </owl:DatatypeProperty>
  <owl:DatatypeProperty rdf:about="http://example.org/onto/prop/google_database_migration_service_connection_profile_database_flags">
    <rdfs:label>database_flags</rdfs:label>
    <rdfs:comment>Database flags to pass to AlloyDB when DMS is creating the AlloyDB cluster and instances. See the AlloyDB documentation for how these can be used.</rdfs:comment>
    <rdfs:domain rdf:resource="http://example.org/onto/class/google_database_migration_service_connection_profile"/>
    <rdfs:range rdf:resource="http://www.w3.org/2001/XMLSchema#string"/>
  </owl:DatatypeProperty>
  <owl:DatatypeProperty rdf:about="http://example.org/onto/prop/google_database_migration_service_connection_profile_id">
    <rdfs:label>id</rdfs:label>
    <rdfs:comment>The database username.</rdfs:comment>
    <rdfs:domain rdf:resource="http://example.org/onto/class/google_database_migration_service_connection_profile"/>
    <rdfs:range rdf:resource="http://www.w3.org/2001/XMLSchema#string"/>
  </owl:DatatypeProperty>
  <owl:DatatypeProperty rdf:about="http://example.org/onto/prop/google_database_migration_service_connection_profile_labels">
    <rdfs:label>labels</rdfs:label>
    <rdfs:comment>Labels for the AlloyDB primary instance created by DMS.</rdfs:comment>
    <rdfs:domain rdf:resource="http://example.org/onto/class/google_database_migration_service_connection_profile"/>
    <rdfs:range rdf:resource="http://www.w3.org/2001/XMLSchema#string"/>
  </owl:DatatypeProperty>
  <owl:DatatypeProperty rdf:about="http://example.org/onto/prop/google_database_migration_service_connection_profile_private_ip">
    <rdfs:label>private_ip</rdfs:label>
    <rdfs:comment>Output only. The private IP address for the Instance. This is the connection endpoint for an end-user application.</rdfs:comment>
    <rdfs:domain rdf:resource="http://example.org/onto/class/google_database_migration_service_connection_profile"/>
    <rdfs:range rdf:resource="http://www.w3.org/2001/XMLSchema#string"/>
  </owl:DatatypeProperty>
  <owl:DatatypeProperty rdf:about="http://example.org/onto/prop/google_database_migration_service_connection_profile_cpu_count">
    <rdfs:label>cpu_count</rdfs:label>
    <rdfs:comment>The number of CPU's in the VM instance.</rdfs:comment>
    <rdfs:domain rdf:resource="http://example.org/onto/class/google_database_migration_service_connection_profile"/>
    <rdfs:range rdf:resource="http://www.w3.org/2001/XMLSchema#string"/>
  </owl:DatatypeProperty>
  <owl:DatatypeProperty rdf:about="http://example.org/onto/prop/google_database_migration_service_connection_profile_cloud_sql_id">
    <rdfs:label>cloud_sql_id</rdfs:label>
    <rdfs:comment>Output only. The Cloud SQL instance ID that this connection profile is associated with.</rdfs:comment>
    <rdfs:domain rdf:resource="http://example.org/onto/class/google_database_migration_service_connection_profile"/>
    <rdfs:range rdf:resource="http://www.w3.org/2001/XMLSchema#string"/>
  </owl:DatatypeProperty>
  <owl:DatatypeProperty rdf:about="http://example.org/onto/prop/google_database_migration_service_connection_profile_private_ip">
    <rdfs:label>private_ip</rdfs:label>
    <rdfs:comment>Output only. The Cloud SQL database instance's private IP.</rdfs:comment>
    <rdfs:domain rdf:resource="http://example.org/onto/class/google_database_migration_service_connection_profile"/>
    <rdfs:range rdf:resource="http://www.w3.org/2001/XMLSchema#string"/>
  </owl:DatatypeProperty>
  <owl:DatatypeProperty rdf:about="http://example.org/onto/prop/google_database_migration_service_connection_profile_public_ip">
    <rdfs:label>public_ip</rdfs:label>
    <rdfs:comment>Output only. The Cloud SQL database instance's public IP.</rdfs:comment>
    <rdfs:domain rdf:resource="http://example.org/onto/class/google_database_migration_service_connection_profile"/>
    <rdfs:range rdf:resource="http://www.w3.org/2001/XMLSchema#string"/>
  </owl:DatatypeProperty>
  <owl:DatatypeProperty rdf:about="http://example.org/onto/prop/google_database_migration_service_connection_profile_activation_policy">
    <rdfs:label>activation_policy</rdfs:label>
    <rdfs:comment>The activation policy specifies when the instance is activated; it is applicable only when the instance state is 'RUNNABLE'. Possible values: ["ALWAYS", "NEVER"]</rdfs:comment>
    <rdfs:domain rdf:resource="http://example.org/onto/class/google_database_migration_service_connection_profile"/>
    <rdfs:range rdf:resource="http://www.w3.org/2001/XMLSchema#string"/>
  </owl:DatatypeProperty>
  <owl:DatatypeProperty rdf:about="http://example.org/onto/prop/google_database_migration_service_connection_profile_auto_storage_increase">
    <rdfs:label>auto_storage_increase</rdfs:label>
    <rdfs:comment>If you enable this setting, Cloud SQL checks your available storage every 30 seconds. If the available storage falls below a threshold size, Cloud SQL automatically adds additional storage capacity.
If the available storage repeatedly falls below the threshold size, Cloud SQL continues to add storage until it reaches the maximum of 30 TB.</rdfs:comment>
    <rdfs:domain rdf:resource="http://example.org/onto/class/google_database_migration_service_connection_profile"/>
    <rdfs:range rdf:resource="http://www.w3.org/2001/XMLSchema#string"/>
  </owl:DatatypeProperty>
  <owl:DatatypeProperty rdf:about="http://example.org/onto/prop/google_database_migration_service_connection_profile_cmek_key_name">
    <rdfs:label>cmek_key_name</rdfs:label>
    <rdfs:comment>The KMS key name used for the csql instance.</rdfs:comment>
    <rdfs:domain rdf:resource="http://example.org/onto/class/google_database_migration_service_connection_profile"/>
    <rdfs:range rdf:resource="http://www.w3.org/2001/XMLSchema#string"/>
  </owl:DatatypeProperty>
  <owl:DatatypeProperty rdf:about="http://example.org/onto/prop/google_database_migration_service_connection_profile_collation">
    <rdfs:label>collation</rdfs:label>
    <rdfs:comment>The Cloud SQL default instance level collation.</rdfs:comment>
    <rdfs:domain rdf:resource="http://example.org/onto/class/google_database_migration_service_connection_profile"/>
    <rdfs:range rdf:resource="http://www.w3.org/2001/XMLSchema#string"/>
  </owl:DatatypeProperty>
  <owl:DatatypeProperty rdf:about="http://example.org/onto/prop/google_database_migration_service_connection_profile_data_disk_size_gb">
    <rdfs:label>data_disk_size_gb</rdfs:label>
    <rdfs:comment>The storage capacity available to the database, in GB. The minimum (and default) size is 10GB.</rdfs:comment>
    <rdfs:domain rdf:resource="http://example.org/onto/class/google_database_migration_service_connection_profile"/>
    <rdfs:range rdf:resource="http://www.w3.org/2001/XMLSchema#string"/>
  </owl:DatatypeProperty>
  <owl:DatatypeProperty rdf:about="http://example.org/onto/prop/google_database_migration_service_connection_profile_data_disk_type">
    <rdfs:label>data_disk_type</rdfs:label>
    <rdfs:comment>The type of storage. Possible values: ["PD_SSD", "PD_HDD"]</rdfs:comment>
    <rdfs:domain rdf:resource="http://example.org/onto/class/google_database_migration_service_connection_profile"/>
    <rdfs:range rdf:resource="http://www.w3.org/2001/XMLSchema#string"/>
  </owl:DatatypeProperty>
  <owl:DatatypeProperty rdf:about="http://example.org/onto/prop/google_database_migration_service_connection_profile_database_flags">
    <rdfs:label>database_flags</rdfs:label>
    <rdfs:comment>The database flags passed to the Cloud SQL instance at startup.</rdfs:comment>
    <rdfs:domain rdf:resource="http://example.org/onto/class/google_database_migration_service_connection_profile"/>
    <rdfs:range rdf:resource="http://www.w3.org/2001/XMLSchema#string"/>
  </owl:DatatypeProperty>
  <owl:DatatypeProperty rdf:about="http://example.org/onto/prop/google_database_migration_service_connection_profile_database_version">
    <rdfs:label>database_version</rdfs:label>
    <rdfs:comment>The database engine type and version.
Currently supported values located at https://cloud.google.com/database-migration/docs/reference/rest/v1/projects.locations.connectionProfiles#sqldatabaseversion</rdfs:comment>
    <rdfs:domain rdf:resource="http://example.org/onto/class/google_database_migration_service_connection_profile"/>
    <rdfs:range rdf:resource="http://www.w3.org/2001/XMLSchema#string"/>
  </owl:DatatypeProperty>
  <owl:DatatypeProperty rdf:about="http://example.org/onto/prop/google_database_migration_service_connection_profile_edition">
    <rdfs:label>edition</rdfs:label>
    <rdfs:comment>The edition of the given Cloud SQL instance. Possible values: ["ENTERPRISE", "ENTERPRISE_PLUS"]</rdfs:comment>
    <rdfs:domain rdf:resource="http://example.org/onto/class/google_database_migration_service_connection_profile"/>
    <rdfs:range rdf:resource="http://www.w3.org/2001/XMLSchema#string"/>
  </owl:DatatypeProperty>
  <owl:DatatypeProperty rdf:about="http://example.org/onto/prop/google_database_migration_service_connection_profile_root_password">
    <rdfs:label>root_password</rdfs:label>
    <rdfs:comment>Input only. Initial root password.</rdfs:comment>
    <rdfs:domain rdf:resource="http://example.org/onto/class/google_database_migration_service_connection_profile"/>
    <rdfs:range rdf:resource="http://www.w3.org/2001/XMLSchema#string"/>
  </owl:DatatypeProperty>
  <owl:DatatypeProperty rdf:about="http://example.org/onto/prop/google_database_migration_service_connection_profile_root_password_set">
    <rdfs:label>root_password_set</rdfs:label>
    <rdfs:comment>Output only. Indicates If this connection profile root password is stored.</rdfs:comment>
    <rdfs:domain rdf:resource="http://example.org/onto/class/google_database_migration_service_connection_profile"/>
    <rdfs:range rdf:resource="http://www.w3.org/2001/XMLSchema#string"/>
  </owl:DatatypeProperty>
  <owl:DatatypeProperty rdf:about="http://example.org/onto/prop/google_database_migration_service_connection_profile_source_id">
    <rdfs:label>source_id</rdfs:label>
    <rdfs:comment>The Database Migration Service source connection profile ID, in the format: projects/my_project_name/locations/us-central1/connectionProfiles/connection_profile_ID</rdfs:comment>
    <rdfs:domain rdf:resource="http://example.org/onto/class/google_database_migration_service_connection_profile"/>
    <rdfs:range rdf:resource="http://www.w3.org/2001/XMLSchema#string"/>
  </owl:DatatypeProperty>
  <owl:DatatypeProperty rdf:about="http://example.org/onto/prop/google_database_migration_service_connection_profile_storage_auto_resize_limit">
    <rdfs:label>storage_auto_resize_limit</rdfs:label>
    <rdfs:comment>The maximum size to which storage capacity can be automatically increased. The default value is 0, which specifies that there is no limit.</rdfs:comment>
    <rdfs:domain rdf:resource="http://example.org/onto/class/google_database_migration_service_connection_profile"/>
    <rdfs:range rdf:resource="http://www.w3.org/2001/XMLSchema#string"/>
  </owl:DatatypeProperty>
  <owl:DatatypeProperty rdf:about="http://example.org/onto/prop/google_database_migration_service_connection_profile_tier">
    <rdfs:label>tier</rdfs:label>
    <rdfs:comment>The tier (or machine type) for this instance, for example: db-n1-standard-1 (MySQL instances) or db-custom-1-3840 (PostgreSQL instances).
For more information, see https://cloud.google.com/sql/docs/mysql/instance-settings</rdfs:comment>
    <rdfs:domain rdf:resource="http://example.org/onto/class/google_database_migration_service_connection_profile"/>
    <rdfs:range rdf:resource="http://www.w3.org/2001/XMLSchema#string"/>
  </owl:DatatypeProperty>
  <owl:DatatypeProperty rdf:about="http://example.org/onto/prop/google_database_migration_service_connection_profile_user_labels">
    <rdfs:label>user_labels</rdfs:label>
    <rdfs:comment>The resource labels for a Cloud SQL instance to use to annotate any related underlying resources such as Compute Engine VMs.</rdfs:comment>
    <rdfs:domain rdf:resource="http://example.org/onto/class/google_database_migration_service_connection_profile"/>
    <rdfs:range rdf:resource="http://www.w3.org/2001/XMLSchema#string"/>
  </owl:DatatypeProperty>
  <owl:DatatypeProperty rdf:about="http://example.org/onto/prop/google_database_migration_service_connection_profile_zone">
    <rdfs:label>zone</rdfs:label>
    <rdfs:comment>The Google Cloud Platform zone where your Cloud SQL datdabse instance is located.</rdfs:comment>
    <rdfs:domain rdf:resource="http://example.org/onto/class/google_database_migration_service_connection_profile"/>
    <rdfs:range rdf:resource="http://www.w3.org/2001/XMLSchema#string"/>
  </owl:DatatypeProperty>
  <owl:DatatypeProperty rdf:about="http://example.org/onto/prop/google_database_migration_service_connection_profile_enable_ipv4">
    <rdfs:label>enable_ipv4</rdfs:label>
    <rdfs:comment>Whether the instance should be assigned an IPv4 address or not.</rdfs:comment>
    <rdfs:domain rdf:resource="http://example.org/onto/class/google_database_migration_service_connection_profile"/>
    <rdfs:range rdf:resource="http://www.w3.org/2001/XMLSchema#string"/>
  </owl:DatatypeProperty>
  <owl:DatatypeProperty rdf:about="http://example.org/onto/prop/google_database_migration_service_connection_profile_private_network">
    <rdfs:label>private_network</rdfs:label>
    <rdfs:comment>The resource link for the VPC network from which the Cloud SQL instance is accessible for private IP. For example, projects/myProject/global/networks/default.
This setting can be updated, but it cannot be removed after it is set.</rdfs:comment>
    <rdfs:domain rdf:resource="http://example.org/onto/class/google_database_migration_service_connection_profile"/>
    <rdfs:range rdf:resource="http://www.w3.org/2001/XMLSchema#string"/>
  </owl:DatatypeProperty>
  <owl:DatatypeProperty rdf:about="http://example.org/onto/prop/google_database_migration_service_connection_profile_require_ssl">
    <rdfs:label>require_ssl</rdfs:label>
    <rdfs:comment>Whether SSL connections over IP should be enforced or not.</rdfs:comment>
    <rdfs:domain rdf:resource="http://example.org/onto/class/google_database_migration_service_connection_profile"/>
    <rdfs:range rdf:resource="http://www.w3.org/2001/XMLSchema#string"/>
  </owl:DatatypeProperty>
  <owl:DatatypeProperty rdf:about="http://example.org/onto/prop/google_database_migration_service_connection_profile_expire_time">
    <rdfs:label>expire_time</rdfs:label>
    <rdfs:comment>The time when this access control entry expires in RFC 3339 format.</rdfs:comment>
    <rdfs:domain rdf:resource="http://example.org/onto/class/google_database_migration_service_connection_profile"/>
    <rdfs:range rdf:resource="http://www.w3.org/2001/XMLSchema#string"/>
  </owl:DatatypeProperty>
  <owl:DatatypeProperty rdf:about="http://example.org/onto/prop/google_database_migration_service_connection_profile_label">
    <rdfs:label>label</rdfs:label>
    <rdfs:comment>A label to identify this entry.</rdfs:comment>
    <rdfs:domain rdf:resource="http://example.org/onto/class/google_database_migration_service_connection_profile"/>
    <rdfs:range rdf:resource="http://www.w3.org/2001/XMLSchema#string"/>
  </owl:DatatypeProperty>
  <owl:DatatypeProperty rdf:about="http://example.org/onto/prop/google_database_migration_service_connection_profile_ttl">
    <rdfs:label>ttl</rdfs:label>
    <rdfs:comment>Input only. The time-to-leave of this access control entry.</rdfs:comment>
    <rdfs:domain rdf:resource="http://example.org/onto/class/google_database_migration_service_connection_profile"/>
    <rdfs:range rdf:resource="http://www.w3.org/2001/XMLSchema#string"/>
  </owl:DatatypeProperty>
  <owl:DatatypeProperty rdf:about="http://example.org/onto/prop/google_database_migration_service_connection_profile_value">
    <rdfs:label>value</rdfs:label>
    <rdfs:comment>The allowlisted value for the access control list.</rdfs:comment>
    <rdfs:domain rdf:resource="http://example.org/onto/class/google_database_migration_service_connection_profile"/>
    <rdfs:range rdf:resource="http://www.w3.org/2001/XMLSchema#string"/>
  </owl:DatatypeProperty>
  <owl:DatatypeProperty rdf:about="http://example.org/onto/prop/google_database_migration_service_connection_profile_cloud_sql_id">
    <rdfs:label>cloud_sql_id</rdfs:label>
    <rdfs:comment>If the source is a Cloud SQL database, use this field to provide the Cloud SQL instance ID of the source.</rdfs:comment>
    <rdfs:domain rdf:resource="http://example.org/onto/class/google_database_migration_service_connection_profile"/>
    <rdfs:range rdf:resource="http://www.w3.org/2001/XMLSchema#string"/>
  </owl:DatatypeProperty>
  <owl:DatatypeProperty rdf:about="http://example.org/onto/prop/google_database_migration_service_connection_profile_host">
    <rdfs:label>host</rdfs:label>
    <rdfs:comment>The IP or hostname of the source MySQL database.</rdfs:comment>
    <rdfs:domain rdf:resource="http://example.org/onto/class/google_database_migration_service_connection_profile"/>
    <rdfs:range rdf:resource="http://www.w3.org/2001/XMLSchema#string"/>
  </owl:DatatypeProperty>
  <owl:DatatypeProperty rdf:about="http://example.org/onto/prop/google_database_migration_service_connection_profile_password">
    <rdfs:label>password</rdfs:label>
    <rdfs:comment>Input only. The password for the user that Database Migration Service will be using to connect to the database.
This field is not returned on request, and the value is encrypted when stored in Database Migration Service.</rdfs:comment>
    <rdfs:domain rdf:resource="http://example.org/onto/class/google_database_migration_service_connection_profile"/>
    <rdfs:range rdf:resource="http://www.w3.org/2001/XMLSchema#string"/>
  </owl:DatatypeProperty>
  <owl:DatatypeProperty rdf:about="http://example.org/onto/prop/google_database_migration_service_connection_profile_password_set">
    <rdfs:label>password_set</rdfs:label>
    <rdfs:comment>Output only. Indicates If this connection profile password is stored.</rdfs:comment>
    <rdfs:domain rdf:resource="http://example.org/onto/class/google_database_migration_service_connection_profile"/>
    <rdfs:range rdf:resource="http://www.w3.org/2001/XMLSchema#string"/>
  </owl:DatatypeProperty>
  <owl:DatatypeProperty rdf:about="http://example.org/onto/prop/google_database_migration_service_connection_profile_port">
    <rdfs:label>port</rdfs:label>
    <rdfs:comment>The network port of the source MySQL database.</rdfs:comment>
    <rdfs:domain rdf:resource="http://example.org/onto/class/google_database_migration_service_connection_profile"/>
    <rdfs:range rdf:resource="http://www.w3.org/2001/XMLSchema#string"/>
  </owl:DatatypeProperty>
  <owl:DatatypeProperty rdf:about="http://example.org/onto/prop/google_database_migration_service_connection_profile_username">
    <rdfs:label>username</rdfs:label>
    <rdfs:comment>The username that Database Migration Service will use to connect to the database. The value is encrypted when stored in Database Migration Service.</rdfs:comment>
    <rdfs:domain rdf:resource="http://example.org/onto/class/google_database_migration_service_connection_profile"/>
    <rdfs:range rdf:resource="http://www.w3.org/2001/XMLSchema#string"/>
  </owl:DatatypeProperty>
  <owl:DatatypeProperty rdf:about="http://example.org/onto/prop/google_database_migration_service_connection_profile_ca_certificate">
    <rdfs:label>ca_certificate</rdfs:label>
    <rdfs:comment>Input only. The x509 PEM-encoded certificate of the CA that signed the source database server's certificate.
The replica will use this certificate to verify it's connecting to the right host.</rdfs:comment>
    <rdfs:domain rdf:resource="http://example.org/onto/class/google_database_migration_service_connection_profile"/>
    <rdfs:range rdf:resource="http://www.w3.org/2001/XMLSchema#string"/>
  </owl:DatatypeProperty>
  <owl:DatatypeProperty rdf:about="http://example.org/onto/prop/google_database_migration_service_connection_profile_client_certificate">
    <rdfs:label>client_certificate</rdfs:label>
    <rdfs:comment>Input only. The x509 PEM-encoded certificate that will be used by the replica to authenticate against the source database server.
If this field is used then the 'clientKey' field is mandatory</rdfs:comment>
    <rdfs:domain rdf:resource="http://example.org/onto/class/google_database_migration_service_connection_profile"/>
    <rdfs:range rdf:resource="http://www.w3.org/2001/XMLSchema#string"/>
  </owl:DatatypeProperty>
  <owl:DatatypeProperty rdf:about="http://example.org/onto/prop/google_database_migration_service_connection_profile_client_key">
    <rdfs:label>client_key</rdfs:label>
    <rdfs:comment>Input only. The unencrypted PKCS#1 or PKCS#8 PEM-encoded private key associated with the Client Certificate.
If this field is used then the 'clientCertificate' field is mandatory.</rdfs:comment>
    <rdfs:domain rdf:resource="http://example.org/onto/class/google_database_migration_service_connection_profile"/>
    <rdfs:range rdf:resource="http://www.w3.org/2001/XMLSchema#string"/>
  </owl:DatatypeProperty>
  <owl:DatatypeProperty rdf:about="http://example.org/onto/prop/google_database_migration_service_connection_profile_type">
    <rdfs:label>type</rdfs:label>
    <rdfs:comment>The current connection profile state. Possible values: ["SERVER_ONLY", "SERVER_CLIENT", "REQUIRED", "NONE"]</rdfs:comment>
    <rdfs:domain rdf:resource="http://example.org/onto/class/google_database_migration_service_connection_profile"/>
    <rdfs:range rdf:resource="http://www.w3.org/2001/XMLSchema#string"/>
  </owl:DatatypeProperty>
  <owl:DatatypeProperty rdf:about="http://example.org/onto/prop/google_database_migration_service_connection_profile_database_service">
    <rdfs:label>database_service</rdfs:label>
    <rdfs:comment>Required. Database service for the Oracle connection.</rdfs:comment>
    <rdfs:domain rdf:resource="http://example.org/onto/class/google_database_migration_service_connection_profile"/>
    <rdfs:range rdf:resource="http://www.w3.org/2001/XMLSchema#string"/>
  </owl:DatatypeProperty>
  <owl:DatatypeProperty rdf:about="http://example.org/onto/prop/google_database_migration_service_connection_profile_host">
    <rdfs:label>host</rdfs:label>
    <rdfs:comment>Required. The IP or hostname of the source Oracle database.</rdfs:comment>
    <rdfs:domain rdf:resource="http://example.org/onto/class/google_database_migration_service_connection_profile"/>
    <rdfs:range rdf:resource="http://www.w3.org/2001/XMLSchema#string"/>
  </owl:DatatypeProperty>
  <owl:DatatypeProperty rdf:about="http://example.org/onto/prop/google_database_migration_service_connection_profile_password">
    <rdfs:label>password</rdfs:label>
    <rdfs:comment>Required. Input only. The password for the user that Database Migration Service will be using to connect to the database.
This field is not returned on request, and the value is encrypted when stored in Database Migration Service.</rdfs:comment>
    <rdfs:domain rdf:resource="http://example.org/onto/class/google_database_migration_service_connection_profile"/>
    <rdfs:range rdf:resource="http://www.w3.org/2001/XMLSchema#string"/>
  </owl:DatatypeProperty>
  <owl:DatatypeProperty rdf:about="http://example.org/onto/prop/google_database_migration_service_connection_profile_password_set">
    <rdfs:label>password_set</rdfs:label>
    <rdfs:comment>Output only. Indicates If this connection profile password is stored.</rdfs:comment>
    <rdfs:domain rdf:resource="http://example.org/onto/class/google_database_migration_service_connection_profile"/>
    <rdfs:range rdf:resource="http://www.w3.org/2001/XMLSchema#string"/>
  </owl:DatatypeProperty>
  <owl:DatatypeProperty rdf:about="http://example.org/onto/prop/google_database_migration_service_connection_profile_port">
    <rdfs:label>port</rdfs:label>
    <rdfs:comment>Required. The network port of the source Oracle database.</rdfs:comment>
    <rdfs:domain rdf:resource="http://example.org/onto/class/google_database_migration_service_connection_profile"/>
    <rdfs:range rdf:resource="http://www.w3.org/2001/XMLSchema#string"/>
  </owl:DatatypeProperty>
  <owl:DatatypeProperty rdf:about="http://example.org/onto/prop/google_database_migration_service_connection_profile_username">
    <rdfs:label>username</rdfs:label>
    <rdfs:comment>Required. The username that Database Migration Service will use to connect to the database. The value is encrypted when stored in Database Migration Service.</rdfs:comment>
    <rdfs:domain rdf:resource="http://example.org/onto/class/google_database_migration_service_connection_profile"/>
    <rdfs:range rdf:resource="http://www.w3.org/2001/XMLSchema#string"/>
  </owl:DatatypeProperty>
  <owl:DatatypeProperty rdf:about="http://example.org/onto/prop/google_database_migration_service_connection_profile_hostname">
    <rdfs:label>hostname</rdfs:label>
    <rdfs:comment>Required. Hostname for the SSH tunnel.</rdfs:comment>
    <rdfs:domain rdf:resource="http://example.org/onto/class/google_database_migration_service_connection_profile"/>
    <rdfs:range rdf:resource="http://www.w3.org/2001/XMLSchema#string"/>
  </owl:DatatypeProperty>
  <owl:DatatypeProperty rdf:about="http://example.org/onto/prop/google_database_migration_service_connection_profile_password">
    <rdfs:label>password</rdfs:label>
    <rdfs:comment>Input only. SSH password. Only one of 'password' and 'private_key' can be configured.</rdfs:comment>
    <rdfs:domain rdf:resource="http://example.org/onto/class/google_database_migration_service_connection_profile"/>
    <rdfs:range rdf:resource="http://www.w3.org/2001/XMLSchema#string"/>
  </owl:DatatypeProperty>
  <owl:DatatypeProperty rdf:about="http://example.org/onto/prop/google_database_migration_service_connection_profile_port">
    <rdfs:label>port</rdfs:label>
    <rdfs:comment>Port for the SSH tunnel, default value is 22.</rdfs:comment>
    <rdfs:domain rdf:resource="http://example.org/onto/class/google_database_migration_service_connection_profile"/>
    <rdfs:range rdf:resource="http://www.w3.org/2001/XMLSchema#string"/>
  </owl:DatatypeProperty>
  <owl:DatatypeProperty rdf:about="http://example.org/onto/prop/google_database_migration_service_connection_profile_private_key">
    <rdfs:label>private_key</rdfs:label>
    <rdfs:comment>Input only. SSH private key. Only one of 'password' and 'private_key' can be configured.</rdfs:comment>
    <rdfs:domain rdf:resource="http://example.org/onto/class/google_database_migration_service_connection_profile"/>
    <rdfs:range rdf:resource="http://www.w3.org/2001/XMLSchema#string"/>
  </owl:DatatypeProperty>
  <owl:DatatypeProperty rdf:about="http://example.org/onto/prop/google_database_migration_service_connection_profile_username">
    <rdfs:label>username</rdfs:label>
    <rdfs:comment>Required. Username for the SSH tunnel.</rdfs:comment>
    <rdfs:domain rdf:resource="http://example.org/onto/class/google_database_migration_service_connection_profile"/>
    <rdfs:range rdf:resource="http://www.w3.org/2001/XMLSchema#string"/>
  </owl:DatatypeProperty>
  <owl:DatatypeProperty rdf:about="http://example.org/onto/prop/google_database_migration_service_connection_profile_private_connection">
    <rdfs:label>private_connection</rdfs:label>
    <rdfs:comment>Required. The resource name (URI) of the private connection.</rdfs:comment>
    <rdfs:domain rdf:resource="http://example.org/onto/class/google_database_migration_service_connection_profile"/>
    <rdfs:range rdf:resource="http://www.w3.org/2001/XMLSchema#string"/>
  </owl:DatatypeProperty>
  <owl:DatatypeProperty rdf:about="http://example.org/onto/prop/google_database_migration_service_connection_profile_ca_certificate">
    <rdfs:label>ca_certificate</rdfs:label>
    <rdfs:comment>Input only. The x509 PEM-encoded certificate of the CA that signed the source database server's certificate.
The replica will use this certificate to verify it's connecting to the right host.</rdfs:comment>
    <rdfs:domain rdf:resource="http://example.org/onto/class/google_database_migration_service_connection_profile"/>
    <rdfs:range rdf:resource="http://www.w3.org/2001/XMLSchema#string"/>
  </owl:DatatypeProperty>
  <owl:DatatypeProperty rdf:about="http://example.org/onto/prop/google_database_migration_service_connection_profile_client_certificate">
    <rdfs:label>client_certificate</rdfs:label>
    <rdfs:comment>Input only. The x509 PEM-encoded certificate that will be used by the replica to authenticate against the source database server.
If this field is used then the 'clientKey' field is mandatory</rdfs:comment>
    <rdfs:domain rdf:resource="http://example.org/onto/class/google_database_migration_service_connection_profile"/>
    <rdfs:range rdf:resource="http://www.w3.org/2001/XMLSchema#string"/>
  </owl:DatatypeProperty>
  <owl:DatatypeProperty rdf:about="http://example.org/onto/prop/google_database_migration_service_connection_profile_client_key">
    <rdfs:label>client_key</rdfs:label>
    <rdfs:comment>Input only. The unencrypted PKCS#1 or PKCS#8 PEM-encoded private key associated with the Client Certificate.
If this field is used then the 'clientCertificate' field is mandatory.</rdfs:comment>
    <rdfs:domain rdf:resource="http://example.org/onto/class/google_database_migration_service_connection_profile"/>
    <rdfs:range rdf:resource="http://www.w3.org/2001/XMLSchema#string"/>
  </owl:DatatypeProperty>
  <owl:DatatypeProperty rdf:about="http://example.org/onto/prop/google_database_migration_service_connection_profile_type">
    <rdfs:label>type</rdfs:label>
    <rdfs:comment>The current connection profile state.</rdfs:comment>
    <rdfs:domain rdf:resource="http://example.org/onto/class/google_database_migration_service_connection_profile"/>
    <rdfs:range rdf:resource="http://www.w3.org/2001/XMLSchema#string"/>
  </owl:DatatypeProperty>
  <owl:DatatypeProperty rdf:about="http://example.org/onto/prop/google_database_migration_service_connection_profile_alloydb_cluster_id">
    <rdfs:label>alloydb_cluster_id</rdfs:label>
    <rdfs:comment>If the connected database is an AlloyDB instance, use this field to provide the AlloyDB cluster ID.</rdfs:comment>
    <rdfs:domain rdf:resource="http://example.org/onto/class/google_database_migration_service_connection_profile"/>
    <rdfs:range rdf:resource="http://www.w3.org/2001/XMLSchema#string"/>
  </owl:DatatypeProperty>
  <owl:DatatypeProperty rdf:about="http://example.org/onto/prop/google_database_migration_service_connection_profile_cloud_sql_id">
    <rdfs:label>cloud_sql_id</rdfs:label>
    <rdfs:comment>If the source is a Cloud SQL database, use this field to provide the Cloud SQL instance ID of the source.</rdfs:comment>
    <rdfs:domain rdf:resource="http://example.org/onto/class/google_database_migration_service_connection_profile"/>
    <rdfs:range rdf:resource="http://www.w3.org/2001/XMLSchema#string"/>
  </owl:DatatypeProperty>
  <owl:DatatypeProperty rdf:about="http://example.org/onto/prop/google_database_migration_service_connection_profile_host">
    <rdfs:label>host</rdfs:label>
    <rdfs:comment>The IP or hostname of the source MySQL database.</rdfs:comment>
    <rdfs:domain rdf:resource="http://example.org/onto/class/google_database_migration_service_connection_profile"/>
    <rdfs:range rdf:resource="http://www.w3.org/2001/XMLSchema#string"/>
  </owl:DatatypeProperty>
  <owl:DatatypeProperty rdf:about="http://example.org/onto/prop/google_database_migration_service_connection_profile_network_architecture">
    <rdfs:label>network_architecture</rdfs:label>
    <rdfs:comment>Output only. If the source is a Cloud SQL database, this field indicates the network architecture it's associated with.</rdfs:comment>
    <rdfs:domain rdf:resource="http://example.org/onto/class/google_database_migration_service_connection_profile"/>
    <rdfs:range rdf:resource="http://www.w3.org/2001/XMLSchema#string"/>
  </owl:DatatypeProperty>
  <owl:DatatypeProperty rdf:about="http://example.org/onto/prop/google_database_migration_service_connection_profile_password">
    <rdfs:label>password</rdfs:label>
    <rdfs:comment>Input only. The password for the user that Database Migration Service will be using to connect to the database.
This field is not returned on request, and the value is encrypted when stored in Database Migration Service.</rdfs:comment>
    <rdfs:domain rdf:resource="http://example.org/onto/class/google_database_migration_service_connection_profile"/>
    <rdfs:range rdf:resource="http://www.w3.org/2001/XMLSchema#string"/>
  </owl:DatatypeProperty>
  <owl:DatatypeProperty rdf:about="http://example.org/onto/prop/google_database_migration_service_connection_profile_password_set">
    <rdfs:label>password_set</rdfs:label>
    <rdfs:comment>Output only. Indicates If this connection profile password is stored.</rdfs:comment>
    <rdfs:domain rdf:resource="http://example.org/onto/class/google_database_migration_service_connection_profile"/>
    <rdfs:range rdf:resource="http://www.w3.org/2001/XMLSchema#string"/>
  </owl:DatatypeProperty>
  <owl:DatatypeProperty rdf:about="http://example.org/onto/prop/google_database_migration_service_connection_profile_port">
    <rdfs:label>port</rdfs:label>
    <rdfs:comment>The network port of the source MySQL database.</rdfs:comment>
    <rdfs:domain rdf:resource="http://example.org/onto/class/google_database_migration_service_connection_profile"/>
    <rdfs:range rdf:resource="http://www.w3.org/2001/XMLSchema#string"/>
  </owl:DatatypeProperty>
  <owl:DatatypeProperty rdf:about="http://example.org/onto/prop/google_database_migration_service_connection_profile_username">
    <rdfs:label>username</rdfs:label>
    <rdfs:comment>The username that Database Migration Service will use to connect to the database. The value is encrypted when stored in Database Migration Service.</rdfs:comment>
    <rdfs:domain rdf:resource="http://example.org/onto/class/google_database_migration_service_connection_profile"/>
    <rdfs:range rdf:resource="http://www.w3.org/2001/XMLSchema#string"/>
  </owl:DatatypeProperty>
  <owl:DatatypeProperty rdf:about="http://example.org/onto/prop/google_database_migration_service_connection_profile_ca_certificate">
    <rdfs:label>ca_certificate</rdfs:label>
    <rdfs:comment>Input only. The x509 PEM-encoded certificate of the CA that signed the source database server's certificate.
The replica will use this certificate to verify it's connecting to the right host.</rdfs:comment>
    <rdfs:domain rdf:resource="http://example.org/onto/class/google_database_migration_service_connection_profile"/>
    <rdfs:range rdf:resource="http://www.w3.org/2001/XMLSchema#string"/>
  </owl:DatatypeProperty>
  <owl:DatatypeProperty rdf:about="http://example.org/onto/prop/google_database_migration_service_connection_profile_client_certificate">
    <rdfs:label>client_certificate</rdfs:label>
    <rdfs:comment>Input only. The x509 PEM-encoded certificate that will be used by the replica to authenticate against the source database server.
If this field is used then the 'clientKey' field is mandatory</rdfs:comment>
    <rdfs:domain rdf:resource="http://example.org/onto/class/google_database_migration_service_connection_profile"/>
    <rdfs:range rdf:resource="http://www.w3.org/2001/XMLSchema#string"/>
  </owl:DatatypeProperty>
  <owl:DatatypeProperty rdf:about="http://example.org/onto/prop/google_database_migration_service_connection_profile_client_key">
    <rdfs:label>client_key</rdfs:label>
    <rdfs:comment>Input only. The unencrypted PKCS#1 or PKCS#8 PEM-encoded private key associated with the Client Certificate.
If this field is used then the 'clientCertificate' field is mandatory.</rdfs:comment>
    <rdfs:domain rdf:resource="http://example.org/onto/class/google_database_migration_service_connection_profile"/>
    <rdfs:range rdf:resource="http://www.w3.org/2001/XMLSchema#string"/>
  </owl:DatatypeProperty>
  <owl:DatatypeProperty rdf:about="http://example.org/onto/prop/google_database_migration_service_connection_profile_type">
    <rdfs:label>type</rdfs:label>
    <rdfs:comment>The current connection profile state. Possible values: ["SERVER_ONLY", "SERVER_CLIENT", "REQUIRED", "NONE"]</rdfs:comment>
    <rdfs:domain rdf:resource="http://example.org/onto/class/google_database_migration_service_connection_profile"/>
    <rdfs:range rdf:resource="http://www.w3.org/2001/XMLSchema#string"/>
  </owl:DatatypeProperty>
  <owl:DatatypeProperty rdf:about="http://example.org/onto/prop/google_database_migration_service_connection_profile_create">
    <rdfs:label>create</rdfs:label>
    <rdfs:domain rdf:resource="http://example.org/onto/class/google_database_migration_service_connection_profile"/>
    <rdfs:range rdf:resource="http://www.w3.org/2001/XMLSchema#string"/>
  </owl:DatatypeProperty>
  <owl:DatatypeProperty rdf:about="http://example.org/onto/prop/google_database_migration_service_connection_profile_delete">
    <rdfs:label>delete</rdfs:label>
    <rdfs:domain rdf:resource="http://example.org/onto/class/google_database_migration_service_connection_profile"/>
    <rdfs:range rdf:resource="http://www.w3.org/2001/XMLSchema#string"/>
  </owl:DatatypeProperty>
  <owl:DatatypeProperty rdf:about="http://example.org/onto/prop/google_database_migration_service_connection_profile_update">
    <rdfs:label>update</rdfs:label>
    <rdfs:domain rdf:resource="http://example.org/onto/class/google_database_migration_service_connection_profile"/>
    <rdfs:range rdf:resource="http://www.w3.org/2001/XMLSchema#string"/>
  </owl:DatatypeProperty>
</rdf:RDF>
