<?xml version="1.0" encoding="UTF-8"?>
<rdf:RDF
  xmlns:rdf="http://www.w3.org/1999/02/22-rdf-syntax-ns#"
  xmlns:rdfs="http://www.w3.org/2000/01/rdf-schema#"
  xmlns:owl="http://www.w3.org/2002/07/owl#"
  xmlns:xsd="http://www.w3.org/2001/XMLSchema#"
  xml:base="http://example.org/onto/">
  <owl:Class rdf:about="http://example.org/onto/class/google_memcache_instance">
    <rdfs:label>google_memcache_instance</rdfs:label>
    <rdfs:comment>#
#     ***     AUTO GENERATED CODE    ***    Type: MMv1     ***
#
# ----------------------------------------------------------------------------
#
#     This code is generated by Magic Modules using the following:
#
#     Configuration: https:#github.com/GoogleCloudPlatform/magic-modules/tree/main/mmv1/products/memcache/Instance.yaml
#     Template:      https:#github.com/GoogleCloudPlatform/magic-modules/tree/main/mmv1/templates/terraform/resource.html.markdown.tmpl
#
#     DO NOT EDIT this file directly. Any changes made to this file will be
#     overwritten during the next generation cycle.
#
# ----------------------------------------------------------------------------
subcategory: "Memcache"
description: |-
  A Google Cloud Memcache instance.
---</rdfs:comment>
  </owl:Class>
  <owl:DatatypeProperty rdf:about="http://example.org/onto/prop/google_memcache_instance_authorized_network">
    <rdfs:label>authorized_network</rdfs:label>
    <rdfs:comment>The full name of the GCE network to connect the instance to.  If not provided,
'default' will be used.</rdfs:comment>
    <rdfs:domain rdf:resource="http://example.org/onto/class/google_memcache_instance"/>
    <rdfs:range rdf:resource="http://www.w3.org/2001/XMLSchema#string"/>
  </owl:DatatypeProperty>
  <owl:DatatypeProperty rdf:about="http://example.org/onto/prop/google_memcache_instance_create_time">
    <rdfs:label>create_time</rdfs:label>
    <rdfs:comment>Creation timestamp in RFC3339 text format.</rdfs:comment>
    <rdfs:domain rdf:resource="http://example.org/onto/class/google_memcache_instance"/>
    <rdfs:range rdf:resource="http://www.w3.org/2001/XMLSchema#string"/>
  </owl:DatatypeProperty>
  <owl:DatatypeProperty rdf:about="http://example.org/onto/prop/google_memcache_instance_deletion_protection">
    <rdfs:label>deletion_protection</rdfs:label>
    <rdfs:comment>Whether Terraform will be prevented from destroying the instance.
When a 'terraform destroy' or 'terraform apply' would delete the instance,
the command will fail if this field is not set to false in Terraform state.
When the field is set to true or unset in Terraform state, a 'terraform apply'
or 'terraform destroy' that would delete the instance will fail.
When the field is set to false, deleting the instance is allowed.</rdfs:comment>
    <rdfs:domain rdf:resource="http://example.org/onto/class/google_memcache_instance"/>
    <rdfs:range rdf:resource="http://www.w3.org/2001/XMLSchema#string"/>
  </owl:DatatypeProperty>
  <owl:DatatypeProperty rdf:about="http://example.org/onto/prop/google_memcache_instance_discovery_endpoint">
    <rdfs:label>discovery_endpoint</rdfs:label>
    <rdfs:comment>Endpoint for Discovery API</rdfs:comment>
    <rdfs:domain rdf:resource="http://example.org/onto/class/google_memcache_instance"/>
    <rdfs:range rdf:resource="http://www.w3.org/2001/XMLSchema#string"/>
  </owl:DatatypeProperty>
  <owl:DatatypeProperty rdf:about="http://example.org/onto/prop/google_memcache_instance_display_name">
    <rdfs:label>display_name</rdfs:label>
    <rdfs:comment>A user-visible name for the instance.</rdfs:comment>
    <rdfs:domain rdf:resource="http://example.org/onto/class/google_memcache_instance"/>
    <rdfs:range rdf:resource="http://www.w3.org/2001/XMLSchema#string"/>
  </owl:DatatypeProperty>
  <owl:DatatypeProperty rdf:about="http://example.org/onto/prop/google_memcache_instance_effective_labels">
    <rdfs:label>effective_labels</rdfs:label>
    <rdfs:comment>All of labels (key/value pairs) present on the resource in GCP, including the labels configured through Terraform, other clients and services.</rdfs:comment>
    <rdfs:domain rdf:resource="http://example.org/onto/class/google_memcache_instance"/>
    <rdfs:range rdf:resource="http://www.w3.org/2001/XMLSchema#string"/>
  </owl:DatatypeProperty>
  <owl:DatatypeProperty rdf:about="http://example.org/onto/prop/google_memcache_instance_id">
    <rdfs:label>id</rdfs:label>
    <rdfs:domain rdf:resource="http://example.org/onto/class/google_memcache_instance"/>
    <rdfs:range rdf:resource="http://www.w3.org/2001/XMLSchema#string"/>
  </owl:DatatypeProperty>
  <owl:DatatypeProperty rdf:about="http://example.org/onto/prop/google_memcache_instance_labels">
    <rdfs:label>labels</rdfs:label>
    <rdfs:comment>Resource labels to represent user-provided metadata.


**Note**: This field is non-authoritative, and will only manage the labels present in your configuration.
Please refer to the field 'effective_labels' for all of the labels present on the resource.</rdfs:comment>
    <rdfs:domain rdf:resource="http://example.org/onto/class/google_memcache_instance"/>
    <rdfs:range rdf:resource="http://www.w3.org/2001/XMLSchema#string"/>
  </owl:DatatypeProperty>
  <owl:DatatypeProperty rdf:about="http://example.org/onto/prop/google_memcache_instance_maintenance_schedule">
    <rdfs:label>maintenance_schedule</rdfs:label>
    <rdfs:comment>Output only. Published maintenance schedule.</rdfs:comment>
    <rdfs:domain rdf:resource="http://example.org/onto/class/google_memcache_instance"/>
    <rdfs:range rdf:resource="http://www.w3.org/2001/XMLSchema#string"/>
  </owl:DatatypeProperty>
  <owl:DatatypeProperty rdf:about="http://example.org/onto/prop/google_memcache_instance_memcache_full_version">
    <rdfs:label>memcache_full_version</rdfs:label>
    <rdfs:comment>The full version of memcached server running on this instance.</rdfs:comment>
    <rdfs:domain rdf:resource="http://example.org/onto/class/google_memcache_instance"/>
    <rdfs:range rdf:resource="http://www.w3.org/2001/XMLSchema#string"/>
  </owl:DatatypeProperty>
  <owl:DatatypeProperty rdf:about="http://example.org/onto/prop/google_memcache_instance_memcache_nodes">
    <rdfs:label>memcache_nodes</rdfs:label>
    <rdfs:comment>Additional information about the instance state, if available.</rdfs:comment>
    <rdfs:domain rdf:resource="http://example.org/onto/class/google_memcache_instance"/>
    <rdfs:range rdf:resource="http://www.w3.org/2001/XMLSchema#string"/>
  </owl:DatatypeProperty>
  <owl:DatatypeProperty rdf:about="http://example.org/onto/prop/google_memcache_instance_memcache_version">
    <rdfs:label>memcache_version</rdfs:label>
    <rdfs:comment>The major version of Memcached software. If not provided, latest supported version will be used.
Currently the latest supported major version is MEMCACHE_1_5. The minor version will be automatically
determined by our system based on the latest supported minor version. Default value: "MEMCACHE_1_5" Possible values: ["MEMCACHE_1_5", "MEMCACHE_1_6_15"]</rdfs:comment>
    <rdfs:domain rdf:resource="http://example.org/onto/class/google_memcache_instance"/>
    <rdfs:range rdf:resource="http://www.w3.org/2001/XMLSchema#string"/>
  </owl:DatatypeProperty>
  <owl:DatatypeProperty rdf:about="http://example.org/onto/prop/google_memcache_instance_name">
    <rdfs:label>name</rdfs:label>
    <rdfs:comment>The resource name of the instance.</rdfs:comment>
    <rdfs:domain rdf:resource="http://example.org/onto/class/google_memcache_instance"/>
    <rdfs:range rdf:resource="http://www.w3.org/2001/XMLSchema#string"/>
  </owl:DatatypeProperty>
  <owl:DatatypeProperty rdf:about="http://example.org/onto/prop/google_memcache_instance_node_count">
    <rdfs:label>node_count</rdfs:label>
    <rdfs:comment>Number of nodes in the memcache instance.</rdfs:comment>
    <rdfs:domain rdf:resource="http://example.org/onto/class/google_memcache_instance"/>
    <rdfs:range rdf:resource="http://www.w3.org/2001/XMLSchema#string"/>
  </owl:DatatypeProperty>
  <owl:DatatypeProperty rdf:about="http://example.org/onto/prop/google_memcache_instance_project">
    <rdfs:label>project</rdfs:label>
    <rdfs:domain rdf:resource="http://example.org/onto/class/google_memcache_instance"/>
    <rdfs:range rdf:resource="http://www.w3.org/2001/XMLSchema#string"/>
  </owl:DatatypeProperty>
  <owl:DatatypeProperty rdf:about="http://example.org/onto/prop/google_memcache_instance_region">
    <rdfs:label>region</rdfs:label>
    <rdfs:comment>The region of the Memcache instance. If it is not provided, the provider region is used.</rdfs:comment>
    <rdfs:domain rdf:resource="http://example.org/onto/class/google_memcache_instance"/>
    <rdfs:range rdf:resource="http://www.w3.org/2001/XMLSchema#string"/>
  </owl:DatatypeProperty>
  <owl:DatatypeProperty rdf:about="http://example.org/onto/prop/google_memcache_instance_reserved_ip_range_id">
    <rdfs:label>reserved_ip_range_id</rdfs:label>
    <rdfs:comment>Contains the name of allocated IP address ranges associated with
the private service access connection for example, "test-default"
associated with IP range 10.0.0.0/29.</rdfs:comment>
    <rdfs:domain rdf:resource="http://example.org/onto/class/google_memcache_instance"/>
    <rdfs:range rdf:resource="http://www.w3.org/2001/XMLSchema#string"/>
  </owl:DatatypeProperty>
  <owl:DatatypeProperty rdf:about="http://example.org/onto/prop/google_memcache_instance_terraform_labels">
    <rdfs:label>terraform_labels</rdfs:label>
    <rdfs:comment>The combination of labels configured directly on the resource
 and default labels configured on the provider.</rdfs:comment>
    <rdfs:domain rdf:resource="http://example.org/onto/class/google_memcache_instance"/>
    <rdfs:range rdf:resource="http://www.w3.org/2001/XMLSchema#string"/>
  </owl:DatatypeProperty>
  <owl:DatatypeProperty rdf:about="http://example.org/onto/prop/google_memcache_instance_zones">
    <rdfs:label>zones</rdfs:label>
    <rdfs:comment>Zones where memcache nodes should be provisioned.  If not
provided, all zones will be used.</rdfs:comment>
    <rdfs:domain rdf:resource="http://example.org/onto/class/google_memcache_instance"/>
    <rdfs:range rdf:resource="http://www.w3.org/2001/XMLSchema#string"/>
  </owl:DatatypeProperty>
  <owl:DatatypeProperty rdf:about="http://example.org/onto/prop/google_memcache_instance_create_time">
    <rdfs:label>create_time</rdfs:label>
    <rdfs:comment>Output only. The time when the policy was created.
A timestamp in RFC3339 UTC "Zulu" format, with nanosecond
resolution and up to nine fractional digits</rdfs:comment>
    <rdfs:domain rdf:resource="http://example.org/onto/class/google_memcache_instance"/>
    <rdfs:range rdf:resource="http://www.w3.org/2001/XMLSchema#string"/>
  </owl:DatatypeProperty>
  <owl:DatatypeProperty rdf:about="http://example.org/onto/prop/google_memcache_instance_description">
    <rdfs:label>description</rdfs:label>
    <rdfs:comment>Optional. Description of what this policy is for.
Create/Update methods return INVALID_ARGUMENT if the
length is greater than 512.</rdfs:comment>
    <rdfs:domain rdf:resource="http://example.org/onto/class/google_memcache_instance"/>
    <rdfs:range rdf:resource="http://www.w3.org/2001/XMLSchema#string"/>
  </owl:DatatypeProperty>
  <owl:DatatypeProperty rdf:about="http://example.org/onto/prop/google_memcache_instance_update_time">
    <rdfs:label>update_time</rdfs:label>
    <rdfs:comment>Output only. The time when the policy was updated.
A timestamp in RFC3339 UTC "Zulu" format, with nanosecond
resolution and up to nine fractional digits.</rdfs:comment>
    <rdfs:domain rdf:resource="http://example.org/onto/class/google_memcache_instance"/>
    <rdfs:range rdf:resource="http://www.w3.org/2001/XMLSchema#string"/>
  </owl:DatatypeProperty>
  <owl:DatatypeProperty rdf:about="http://example.org/onto/prop/google_memcache_instance_day">
    <rdfs:label>day</rdfs:label>
    <rdfs:comment>Required. The day of week that maintenance updates occur.
- DAY_OF_WEEK_UNSPECIFIED: The day of the week is unspecified.
- MONDAY: Monday
- TUESDAY: Tuesday
- WEDNESDAY: Wednesday
- THURSDAY: Thursday
- FRIDAY: Friday
- SATURDAY: Saturday
- SUNDAY: Sunday Possible values: ["DAY_OF_WEEK_UNSPECIFIED", "MONDAY", "TUESDAY", "WEDNESDAY", "THURSDAY", "FRIDAY", "SATURDAY", "SUNDAY"]</rdfs:comment>
    <rdfs:domain rdf:resource="http://example.org/onto/class/google_memcache_instance"/>
    <rdfs:range rdf:resource="http://www.w3.org/2001/XMLSchema#string"/>
  </owl:DatatypeProperty>
  <owl:DatatypeProperty rdf:about="http://example.org/onto/prop/google_memcache_instance_duration">
    <rdfs:label>duration</rdfs:label>
    <rdfs:comment>Required. The length of the maintenance window, ranging from 3 hours to 8 hours.
A duration in seconds with up to nine fractional digits,
terminated by 's'. Example: "3.5s".</rdfs:comment>
    <rdfs:domain rdf:resource="http://example.org/onto/class/google_memcache_instance"/>
    <rdfs:range rdf:resource="http://www.w3.org/2001/XMLSchema#string"/>
  </owl:DatatypeProperty>
  <owl:DatatypeProperty rdf:about="http://example.org/onto/prop/google_memcache_instance_hours">
    <rdfs:label>hours</rdfs:label>
    <rdfs:comment>Hours of day in 24 hour format. Should be from 0 to 23.
An API may choose to allow the value "24:00:00" for scenarios like business closing time.</rdfs:comment>
    <rdfs:domain rdf:resource="http://example.org/onto/class/google_memcache_instance"/>
    <rdfs:range rdf:resource="http://www.w3.org/2001/XMLSchema#string"/>
  </owl:DatatypeProperty>
  <owl:DatatypeProperty rdf:about="http://example.org/onto/prop/google_memcache_instance_minutes">
    <rdfs:label>minutes</rdfs:label>
    <rdfs:comment>Minutes of hour of day. Must be from 0 to 59.</rdfs:comment>
    <rdfs:domain rdf:resource="http://example.org/onto/class/google_memcache_instance"/>
    <rdfs:range rdf:resource="http://www.w3.org/2001/XMLSchema#string"/>
  </owl:DatatypeProperty>
  <owl:DatatypeProperty rdf:about="http://example.org/onto/prop/google_memcache_instance_nanos">
    <rdfs:label>nanos</rdfs:label>
    <rdfs:comment>Fractions of seconds in nanoseconds. Must be from 0 to 999,999,999.</rdfs:comment>
    <rdfs:domain rdf:resource="http://example.org/onto/class/google_memcache_instance"/>
    <rdfs:range rdf:resource="http://www.w3.org/2001/XMLSchema#string"/>
  </owl:DatatypeProperty>
  <owl:DatatypeProperty rdf:about="http://example.org/onto/prop/google_memcache_instance_seconds">
    <rdfs:label>seconds</rdfs:label>
    <rdfs:comment>Seconds of minutes of the time. Must normally be from 0 to 59.
An API may allow the value 60 if it allows leap-seconds.</rdfs:comment>
    <rdfs:domain rdf:resource="http://example.org/onto/class/google_memcache_instance"/>
    <rdfs:range rdf:resource="http://www.w3.org/2001/XMLSchema#string"/>
  </owl:DatatypeProperty>
  <owl:DatatypeProperty rdf:about="http://example.org/onto/prop/google_memcache_instance_id">
    <rdfs:label>id</rdfs:label>
    <rdfs:comment>This is a unique ID associated with this set of parameters.</rdfs:comment>
    <rdfs:domain rdf:resource="http://example.org/onto/class/google_memcache_instance"/>
    <rdfs:range rdf:resource="http://www.w3.org/2001/XMLSchema#string"/>
  </owl:DatatypeProperty>
  <owl:DatatypeProperty rdf:about="http://example.org/onto/prop/google_memcache_instance_params">
    <rdfs:label>params</rdfs:label>
    <rdfs:comment>User-defined set of parameters to use in the memcache process.</rdfs:comment>
    <rdfs:domain rdf:resource="http://example.org/onto/class/google_memcache_instance"/>
    <rdfs:range rdf:resource="http://www.w3.org/2001/XMLSchema#string"/>
  </owl:DatatypeProperty>
  <owl:DatatypeProperty rdf:about="http://example.org/onto/prop/google_memcache_instance_cpu_count">
    <rdfs:label>cpu_count</rdfs:label>
    <rdfs:comment>Number of CPUs per node.</rdfs:comment>
    <rdfs:domain rdf:resource="http://example.org/onto/class/google_memcache_instance"/>
    <rdfs:range rdf:resource="http://www.w3.org/2001/XMLSchema#string"/>
  </owl:DatatypeProperty>
  <owl:DatatypeProperty rdf:about="http://example.org/onto/prop/google_memcache_instance_memory_size_mb">
    <rdfs:label>memory_size_mb</rdfs:label>
    <rdfs:comment>Memory size in Mebibytes for each memcache node.</rdfs:comment>
    <rdfs:domain rdf:resource="http://example.org/onto/class/google_memcache_instance"/>
    <rdfs:range rdf:resource="http://www.w3.org/2001/XMLSchema#string"/>
  </owl:DatatypeProperty>
  <owl:DatatypeProperty rdf:about="http://example.org/onto/prop/google_memcache_instance_create">
    <rdfs:label>create</rdfs:label>
    <rdfs:domain rdf:resource="http://example.org/onto/class/google_memcache_instance"/>
    <rdfs:range rdf:resource="http://www.w3.org/2001/XMLSchema#string"/>
  </owl:DatatypeProperty>
  <owl:DatatypeProperty rdf:about="http://example.org/onto/prop/google_memcache_instance_delete">
    <rdfs:label>delete</rdfs:label>
    <rdfs:domain rdf:resource="http://example.org/onto/class/google_memcache_instance"/>
    <rdfs:range rdf:resource="http://www.w3.org/2001/XMLSchema#string"/>
  </owl:DatatypeProperty>
  <owl:DatatypeProperty rdf:about="http://example.org/onto/prop/google_memcache_instance_update">
    <rdfs:label>update</rdfs:label>
    <rdfs:domain rdf:resource="http://example.org/onto/class/google_memcache_instance"/>
    <rdfs:range rdf:resource="http://www.w3.org/2001/XMLSchema#string"/>
  </owl:DatatypeProperty>
</rdf:RDF>
