<?xml version="1.0" encoding="UTF-8"?>
<rdf:RDF
  xmlns:rdf="http://www.w3.org/1999/02/22-rdf-syntax-ns#"
  xmlns:rdfs="http://www.w3.org/2000/01/rdf-schema#"
  xmlns:owl="http://www.w3.org/2002/07/owl#"
  xmlns:xsd="http://www.w3.org/2001/XMLSchema#"
  xml:base="http://example.org/onto/">
  <owl:Class rdf:about="http://example.org/onto/class/google_compute_instance_template">
    <rdfs:label>google_compute_instance_template</rdfs:label>
    <rdfs:comment>#
#     ***     AUTO GENERATED CODE    ***    Type: Handwritten     ***
#
# ----------------------------------------------------------------------------
#
#     This code is generated by Magic Modules using the following:
#
#     Source file: https://github.com/GoogleCloudPlatform/magic-modules/tree/main/mmv1/third_party/terraform/website/docs/r/compute_instance_template.html.markdown
#
#     DO NOT EDIT this file directly. Any changes made to this file will be
#     overwritten during the next generation cycle.
#
# ----------------------------------------------------------------------------
subcategory: "Compute Engine"
description: |-
  Manages a VM instance template resource within GCE.
---</rdfs:comment>
  </owl:Class>
  <owl:DatatypeProperty rdf:about="http://example.org/onto/prop/google_compute_instance_template_can_ip_forward">
    <rdfs:label>can_ip_forward</rdfs:label>
    <rdfs:comment>Whether to allow sending and receiving of packets with non-matching source or destination IPs. This defaults to false.</rdfs:comment>
    <rdfs:domain rdf:resource="http://example.org/onto/class/google_compute_instance_template"/>
    <rdfs:range rdf:resource="http://www.w3.org/2001/XMLSchema#string"/>
  </owl:DatatypeProperty>
  <owl:DatatypeProperty rdf:about="http://example.org/onto/prop/google_compute_instance_template_creation_timestamp">
    <rdfs:label>creation_timestamp</rdfs:label>
    <rdfs:comment>Creation timestamp in RFC3339 text format.</rdfs:comment>
    <rdfs:domain rdf:resource="http://example.org/onto/class/google_compute_instance_template"/>
    <rdfs:range rdf:resource="http://www.w3.org/2001/XMLSchema#string"/>
  </owl:DatatypeProperty>
  <owl:DatatypeProperty rdf:about="http://example.org/onto/prop/google_compute_instance_template_description">
    <rdfs:label>description</rdfs:label>
    <rdfs:comment>A brief description of this resource.</rdfs:comment>
    <rdfs:domain rdf:resource="http://example.org/onto/class/google_compute_instance_template"/>
    <rdfs:range rdf:resource="http://www.w3.org/2001/XMLSchema#string"/>
  </owl:DatatypeProperty>
  <owl:DatatypeProperty rdf:about="http://example.org/onto/prop/google_compute_instance_template_effective_labels">
    <rdfs:label>effective_labels</rdfs:label>
    <rdfs:comment>All of labels (key/value pairs) present on the resource in GCP, including the labels configured through Terraform, other clients and services.</rdfs:comment>
    <rdfs:domain rdf:resource="http://example.org/onto/class/google_compute_instance_template"/>
    <rdfs:range rdf:resource="http://www.w3.org/2001/XMLSchema#string"/>
  </owl:DatatypeProperty>
  <owl:DatatypeProperty rdf:about="http://example.org/onto/prop/google_compute_instance_template_id">
    <rdfs:label>id</rdfs:label>
    <rdfs:domain rdf:resource="http://example.org/onto/class/google_compute_instance_template"/>
    <rdfs:range rdf:resource="http://www.w3.org/2001/XMLSchema#string"/>
  </owl:DatatypeProperty>
  <owl:DatatypeProperty rdf:about="http://example.org/onto/prop/google_compute_instance_template_instance_description">
    <rdfs:label>instance_description</rdfs:label>
    <rdfs:comment>A description of the instance.</rdfs:comment>
    <rdfs:domain rdf:resource="http://example.org/onto/class/google_compute_instance_template"/>
    <rdfs:range rdf:resource="http://www.w3.org/2001/XMLSchema#string"/>
  </owl:DatatypeProperty>
  <owl:DatatypeProperty rdf:about="http://example.org/onto/prop/google_compute_instance_template_key_revocation_action_type">
    <rdfs:label>key_revocation_action_type</rdfs:label>
    <rdfs:comment>Action to be taken when a customer's encryption key is revoked. Supports "STOP" and "NONE", with "NONE" being the default.</rdfs:comment>
    <rdfs:domain rdf:resource="http://example.org/onto/class/google_compute_instance_template"/>
    <rdfs:range rdf:resource="http://www.w3.org/2001/XMLSchema#string"/>
  </owl:DatatypeProperty>
  <owl:DatatypeProperty rdf:about="http://example.org/onto/prop/google_compute_instance_template_labels">
    <rdfs:label>labels</rdfs:label>
    <rdfs:comment>A set of key/value label pairs to assign to instances created from this template.

				**Note**: This field is non-authoritative, and will only manage the labels present in your configuration.
				Please refer to the field 'effective_labels' for all of the labels present on the resource.</rdfs:comment>
    <rdfs:domain rdf:resource="http://example.org/onto/class/google_compute_instance_template"/>
    <rdfs:range rdf:resource="http://www.w3.org/2001/XMLSchema#string"/>
  </owl:DatatypeProperty>
  <owl:DatatypeProperty rdf:about="http://example.org/onto/prop/google_compute_instance_template_machine_type">
    <rdfs:label>machine_type</rdfs:label>
    <rdfs:comment>The machine type to create. To create a machine with a custom type (such as extended memory), format the value like custom-VCPUS-MEM_IN_MB like custom-6-20480 for 6 vCPU and 20GB of RAM.</rdfs:comment>
    <rdfs:domain rdf:resource="http://example.org/onto/class/google_compute_instance_template"/>
    <rdfs:range rdf:resource="http://www.w3.org/2001/XMLSchema#string"/>
  </owl:DatatypeProperty>
  <owl:DatatypeProperty rdf:about="http://example.org/onto/prop/google_compute_instance_template_metadata">
    <rdfs:label>metadata</rdfs:label>
    <rdfs:comment>Metadata key/value pairs to make available from within instances created from this template.</rdfs:comment>
    <rdfs:domain rdf:resource="http://example.org/onto/class/google_compute_instance_template"/>
    <rdfs:range rdf:resource="http://www.w3.org/2001/XMLSchema#string"/>
  </owl:DatatypeProperty>
  <owl:DatatypeProperty rdf:about="http://example.org/onto/prop/google_compute_instance_template_metadata_fingerprint">
    <rdfs:label>metadata_fingerprint</rdfs:label>
    <rdfs:comment>The unique fingerprint of the metadata.</rdfs:comment>
    <rdfs:domain rdf:resource="http://example.org/onto/class/google_compute_instance_template"/>
    <rdfs:range rdf:resource="http://www.w3.org/2001/XMLSchema#string"/>
  </owl:DatatypeProperty>
  <owl:DatatypeProperty rdf:about="http://example.org/onto/prop/google_compute_instance_template_metadata_startup_script">
    <rdfs:label>metadata_startup_script</rdfs:label>
    <rdfs:comment>An alternative to using the startup-script metadata key, mostly to match the compute_instance resource. This replaces the startup-script metadata key on the created instance and thus the two mechanisms are not allowed to be used simultaneously.</rdfs:comment>
    <rdfs:domain rdf:resource="http://example.org/onto/class/google_compute_instance_template"/>
    <rdfs:range rdf:resource="http://www.w3.org/2001/XMLSchema#string"/>
  </owl:DatatypeProperty>
  <owl:DatatypeProperty rdf:about="http://example.org/onto/prop/google_compute_instance_template_min_cpu_platform">
    <rdfs:label>min_cpu_platform</rdfs:label>
    <rdfs:comment>Specifies a minimum CPU platform. Applicable values are the friendly names of CPU platforms, such as Intel Haswell or Intel Skylake.</rdfs:comment>
    <rdfs:domain rdf:resource="http://example.org/onto/class/google_compute_instance_template"/>
    <rdfs:range rdf:resource="http://www.w3.org/2001/XMLSchema#string"/>
  </owl:DatatypeProperty>
  <owl:DatatypeProperty rdf:about="http://example.org/onto/prop/google_compute_instance_template_name">
    <rdfs:label>name</rdfs:label>
    <rdfs:comment>The name of the instance template. If you leave this blank, Terraform will auto-generate a unique name.</rdfs:comment>
    <rdfs:domain rdf:resource="http://example.org/onto/class/google_compute_instance_template"/>
    <rdfs:range rdf:resource="http://www.w3.org/2001/XMLSchema#string"/>
  </owl:DatatypeProperty>
  <owl:DatatypeProperty rdf:about="http://example.org/onto/prop/google_compute_instance_template_name_prefix">
    <rdfs:label>name_prefix</rdfs:label>
    <rdfs:comment>Creates a unique name beginning with the specified prefix. Conflicts with name. Max length is 54 characters. Prefixes with lengths longer than 37 characters will use a shortened UUID that will be more prone to collisions.</rdfs:comment>
    <rdfs:domain rdf:resource="http://example.org/onto/class/google_compute_instance_template"/>
    <rdfs:range rdf:resource="http://www.w3.org/2001/XMLSchema#string"/>
  </owl:DatatypeProperty>
  <owl:DatatypeProperty rdf:about="http://example.org/onto/prop/google_compute_instance_template_numeric_id">
    <rdfs:label>numeric_id</rdfs:label>
    <rdfs:comment>The ID of the template in numeric format.</rdfs:comment>
    <rdfs:domain rdf:resource="http://example.org/onto/class/google_compute_instance_template"/>
    <rdfs:range rdf:resource="http://www.w3.org/2001/XMLSchema#string"/>
  </owl:DatatypeProperty>
  <owl:DatatypeProperty rdf:about="http://example.org/onto/prop/google_compute_instance_template_project">
    <rdfs:label>project</rdfs:label>
    <rdfs:comment>The ID of the project in which the resource belongs. If it is not provided, the provider project is used.</rdfs:comment>
    <rdfs:domain rdf:resource="http://example.org/onto/class/google_compute_instance_template"/>
    <rdfs:range rdf:resource="http://www.w3.org/2001/XMLSchema#string"/>
  </owl:DatatypeProperty>
  <owl:DatatypeProperty rdf:about="http://example.org/onto/prop/google_compute_instance_template_region">
    <rdfs:label>region</rdfs:label>
    <rdfs:comment>An instance template is a global resource that is not bound to a zone or a region. However, you can still specify some regional resources in an instance template, which restricts the template to the region where that resource resides. For example, a custom subnetwork resource is tied to a specific region. Defaults to the region of the Provider if no value is given.</rdfs:comment>
    <rdfs:domain rdf:resource="http://example.org/onto/class/google_compute_instance_template"/>
    <rdfs:range rdf:resource="http://www.w3.org/2001/XMLSchema#string"/>
  </owl:DatatypeProperty>
  <owl:DatatypeProperty rdf:about="http://example.org/onto/prop/google_compute_instance_template_resource_manager_tags">
    <rdfs:label>resource_manager_tags</rdfs:label>
    <rdfs:comment>A map of resource manager tags.
				Resource manager tag keys and values have the same definition as resource manager tags.
				Keys must be in the format tagKeys/{tag_key_id}, and values are in the format tagValues/456.
				The field is ignored (both PUT & PATCH) when empty.</rdfs:comment>
    <rdfs:domain rdf:resource="http://example.org/onto/class/google_compute_instance_template"/>
    <rdfs:range rdf:resource="http://www.w3.org/2001/XMLSchema#string"/>
  </owl:DatatypeProperty>
  <owl:DatatypeProperty rdf:about="http://example.org/onto/prop/google_compute_instance_template_resource_policies">
    <rdfs:label>resource_policies</rdfs:label>
    <rdfs:comment>A list of self_links of resource policies to attach to the instance. Currently a max of 1 resource policy is supported.</rdfs:comment>
    <rdfs:domain rdf:resource="http://example.org/onto/class/google_compute_instance_template"/>
    <rdfs:range rdf:resource="http://www.w3.org/2001/XMLSchema#string"/>
  </owl:DatatypeProperty>
  <owl:DatatypeProperty rdf:about="http://example.org/onto/prop/google_compute_instance_template_self_link">
    <rdfs:label>self_link</rdfs:label>
    <rdfs:comment>The URI of the created resource.</rdfs:comment>
    <rdfs:domain rdf:resource="http://example.org/onto/class/google_compute_instance_template"/>
    <rdfs:range rdf:resource="http://www.w3.org/2001/XMLSchema#string"/>
  </owl:DatatypeProperty>
  <owl:DatatypeProperty rdf:about="http://example.org/onto/prop/google_compute_instance_template_self_link_unique">
    <rdfs:label>self_link_unique</rdfs:label>
    <rdfs:comment>A special URI of the created resource that uniquely identifies this instance template.</rdfs:comment>
    <rdfs:domain rdf:resource="http://example.org/onto/class/google_compute_instance_template"/>
    <rdfs:range rdf:resource="http://www.w3.org/2001/XMLSchema#string"/>
  </owl:DatatypeProperty>
  <owl:DatatypeProperty rdf:about="http://example.org/onto/prop/google_compute_instance_template_tags">
    <rdfs:label>tags</rdfs:label>
    <rdfs:comment>Tags to attach to the instance.</rdfs:comment>
    <rdfs:domain rdf:resource="http://example.org/onto/class/google_compute_instance_template"/>
    <rdfs:range rdf:resource="http://www.w3.org/2001/XMLSchema#string"/>
  </owl:DatatypeProperty>
  <owl:DatatypeProperty rdf:about="http://example.org/onto/prop/google_compute_instance_template_tags_fingerprint">
    <rdfs:label>tags_fingerprint</rdfs:label>
    <rdfs:comment>The unique fingerprint of the tags.</rdfs:comment>
    <rdfs:domain rdf:resource="http://example.org/onto/class/google_compute_instance_template"/>
    <rdfs:range rdf:resource="http://www.w3.org/2001/XMLSchema#string"/>
  </owl:DatatypeProperty>
  <owl:DatatypeProperty rdf:about="http://example.org/onto/prop/google_compute_instance_template_terraform_labels">
    <rdfs:label>terraform_labels</rdfs:label>
    <rdfs:comment>The combination of labels configured directly on the resource and default labels configured on the provider.</rdfs:comment>
    <rdfs:domain rdf:resource="http://example.org/onto/class/google_compute_instance_template"/>
    <rdfs:range rdf:resource="http://www.w3.org/2001/XMLSchema#string"/>
  </owl:DatatypeProperty>
  <owl:DatatypeProperty rdf:about="http://example.org/onto/prop/google_compute_instance_template_enable_nested_virtualization">
    <rdfs:label>enable_nested_virtualization</rdfs:label>
    <rdfs:comment>Whether to enable nested virtualization or not.</rdfs:comment>
    <rdfs:domain rdf:resource="http://example.org/onto/class/google_compute_instance_template"/>
    <rdfs:range rdf:resource="http://www.w3.org/2001/XMLSchema#string"/>
  </owl:DatatypeProperty>
  <owl:DatatypeProperty rdf:about="http://example.org/onto/prop/google_compute_instance_template_enable_uefi_networking">
    <rdfs:label>enable_uefi_networking</rdfs:label>
    <rdfs:comment>Whether to enable UEFI networking or not.</rdfs:comment>
    <rdfs:domain rdf:resource="http://example.org/onto/class/google_compute_instance_template"/>
    <rdfs:range rdf:resource="http://www.w3.org/2001/XMLSchema#string"/>
  </owl:DatatypeProperty>
  <owl:DatatypeProperty rdf:about="http://example.org/onto/prop/google_compute_instance_template_performance_monitoring_unit">
    <rdfs:label>performance_monitoring_unit</rdfs:label>
    <rdfs:comment>The PMU is a hardware component within the CPU core that monitors how the processor runs code. Valid values for the level of PMU are "STANDARD", "ENHANCED", and "ARCHITECTURAL".</rdfs:comment>
    <rdfs:domain rdf:resource="http://example.org/onto/class/google_compute_instance_template"/>
    <rdfs:range rdf:resource="http://www.w3.org/2001/XMLSchema#string"/>
  </owl:DatatypeProperty>
  <owl:DatatypeProperty rdf:about="http://example.org/onto/prop/google_compute_instance_template_threads_per_core">
    <rdfs:label>threads_per_core</rdfs:label>
    <rdfs:comment>The number of threads per physical core. To disable simultaneous multithreading (SMT) set this to 1. If unset, the maximum number of threads supported per core by the underlying processor is assumed.</rdfs:comment>
    <rdfs:domain rdf:resource="http://example.org/onto/class/google_compute_instance_template"/>
    <rdfs:range rdf:resource="http://www.w3.org/2001/XMLSchema#string"/>
  </owl:DatatypeProperty>
  <owl:DatatypeProperty rdf:about="http://example.org/onto/prop/google_compute_instance_template_turbo_mode">
    <rdfs:label>turbo_mode</rdfs:label>
    <rdfs:comment>Turbo frequency mode to use for the instance. Currently supported modes is "ALL_CORE_MAX".</rdfs:comment>
    <rdfs:domain rdf:resource="http://example.org/onto/class/google_compute_instance_template"/>
    <rdfs:range rdf:resource="http://www.w3.org/2001/XMLSchema#string"/>
  </owl:DatatypeProperty>
  <owl:DatatypeProperty rdf:about="http://example.org/onto/prop/google_compute_instance_template_visible_core_count">
    <rdfs:label>visible_core_count</rdfs:label>
    <rdfs:comment>The number of physical cores to expose to an instance. Multiply by the number of threads per core to compute the total number of virtual CPUs to expose to the instance. If unset, the number of cores is inferred from the instance\'s nominal CPU count and the underlying platform\'s SMT width.</rdfs:comment>
    <rdfs:domain rdf:resource="http://example.org/onto/class/google_compute_instance_template"/>
    <rdfs:range rdf:resource="http://www.w3.org/2001/XMLSchema#string"/>
  </owl:DatatypeProperty>
  <owl:DatatypeProperty rdf:about="http://example.org/onto/prop/google_compute_instance_template_confidential_instance_type">
    <rdfs:label>confidential_instance_type</rdfs:label>
    <rdfs:comment>The confidential computing technology the instance uses.
								SEV is an AMD feature. TDX is an Intel feature. One of the following
								values is required: SEV, SEV_SNP, TDX. If SEV_SNP, min_cpu_platform =
								"AMD Milan" is currently required.</rdfs:comment>
    <rdfs:domain rdf:resource="http://example.org/onto/class/google_compute_instance_template"/>
    <rdfs:range rdf:resource="http://www.w3.org/2001/XMLSchema#string"/>
  </owl:DatatypeProperty>
  <owl:DatatypeProperty rdf:about="http://example.org/onto/prop/google_compute_instance_template_enable_confidential_compute">
    <rdfs:label>enable_confidential_compute</rdfs:label>
    <rdfs:comment>Defines whether the instance should have confidential compute enabled. Field will be deprecated in a future release.</rdfs:comment>
    <rdfs:domain rdf:resource="http://example.org/onto/class/google_compute_instance_template"/>
    <rdfs:range rdf:resource="http://www.w3.org/2001/XMLSchema#string"/>
  </owl:DatatypeProperty>
  <owl:DatatypeProperty rdf:about="http://example.org/onto/prop/google_compute_instance_template_architecture">
    <rdfs:label>architecture</rdfs:label>
    <rdfs:comment>The architecture of the image. Allowed values are ARM64 or X86_64.</rdfs:comment>
    <rdfs:domain rdf:resource="http://example.org/onto/class/google_compute_instance_template"/>
    <rdfs:range rdf:resource="http://www.w3.org/2001/XMLSchema#string"/>
  </owl:DatatypeProperty>
  <owl:DatatypeProperty rdf:about="http://example.org/onto/prop/google_compute_instance_template_auto_delete">
    <rdfs:label>auto_delete</rdfs:label>
    <rdfs:comment>Whether or not the disk should be auto-deleted. This defaults to true.</rdfs:comment>
    <rdfs:domain rdf:resource="http://example.org/onto/class/google_compute_instance_template"/>
    <rdfs:range rdf:resource="http://www.w3.org/2001/XMLSchema#string"/>
  </owl:DatatypeProperty>
  <owl:DatatypeProperty rdf:about="http://example.org/onto/prop/google_compute_instance_template_boot">
    <rdfs:label>boot</rdfs:label>
    <rdfs:comment>Indicates that this is a boot disk.</rdfs:comment>
    <rdfs:domain rdf:resource="http://example.org/onto/class/google_compute_instance_template"/>
    <rdfs:range rdf:resource="http://www.w3.org/2001/XMLSchema#string"/>
  </owl:DatatypeProperty>
  <owl:DatatypeProperty rdf:about="http://example.org/onto/prop/google_compute_instance_template_device_name">
    <rdfs:label>device_name</rdfs:label>
    <rdfs:comment>A unique device name that is reflected into the /dev/ tree of a Linux operating system running within the instance. If not specified, the server chooses a default device name to apply to this disk.</rdfs:comment>
    <rdfs:domain rdf:resource="http://example.org/onto/class/google_compute_instance_template"/>
    <rdfs:range rdf:resource="http://www.w3.org/2001/XMLSchema#string"/>
  </owl:DatatypeProperty>
  <owl:DatatypeProperty rdf:about="http://example.org/onto/prop/google_compute_instance_template_disk_name">
    <rdfs:label>disk_name</rdfs:label>
    <rdfs:comment>Name of the disk. When not provided, this defaults to the name of the instance.</rdfs:comment>
    <rdfs:domain rdf:resource="http://example.org/onto/class/google_compute_instance_template"/>
    <rdfs:range rdf:resource="http://www.w3.org/2001/XMLSchema#string"/>
  </owl:DatatypeProperty>
  <owl:DatatypeProperty rdf:about="http://example.org/onto/prop/google_compute_instance_template_disk_size_gb">
    <rdfs:label>disk_size_gb</rdfs:label>
    <rdfs:comment>The size of the image in gigabytes. If not specified, it will inherit the size of its base image. For SCRATCH disks, the size must be one of 375 or 3000 GB, with a default of 375 GB.</rdfs:comment>
    <rdfs:domain rdf:resource="http://example.org/onto/class/google_compute_instance_template"/>
    <rdfs:range rdf:resource="http://www.w3.org/2001/XMLSchema#string"/>
  </owl:DatatypeProperty>
  <owl:DatatypeProperty rdf:about="http://example.org/onto/prop/google_compute_instance_template_disk_type">
    <rdfs:label>disk_type</rdfs:label>
    <rdfs:comment>The Google Compute Engine disk type. Such as "pd-ssd", "local-ssd", "pd-balanced" or "pd-standard".</rdfs:comment>
    <rdfs:domain rdf:resource="http://example.org/onto/class/google_compute_instance_template"/>
    <rdfs:range rdf:resource="http://www.w3.org/2001/XMLSchema#string"/>
  </owl:DatatypeProperty>
  <owl:DatatypeProperty rdf:about="http://example.org/onto/prop/google_compute_instance_template_guest_os_features">
    <rdfs:label>guest_os_features</rdfs:label>
    <rdfs:comment>A list of features to enable on the guest operating system. Applicable only for bootable images.</rdfs:comment>
    <rdfs:domain rdf:resource="http://example.org/onto/class/google_compute_instance_template"/>
    <rdfs:range rdf:resource="http://www.w3.org/2001/XMLSchema#string"/>
  </owl:DatatypeProperty>
  <owl:DatatypeProperty rdf:about="http://example.org/onto/prop/google_compute_instance_template_interface">
    <rdfs:label>interface</rdfs:label>
    <rdfs:comment>Specifies the disk interface to use for attaching this disk.</rdfs:comment>
    <rdfs:domain rdf:resource="http://example.org/onto/class/google_compute_instance_template"/>
    <rdfs:range rdf:resource="http://www.w3.org/2001/XMLSchema#string"/>
  </owl:DatatypeProperty>
  <owl:DatatypeProperty rdf:about="http://example.org/onto/prop/google_compute_instance_template_labels">
    <rdfs:label>labels</rdfs:label>
    <rdfs:comment>A set of key/value label pairs to assign to disks,</rdfs:comment>
    <rdfs:domain rdf:resource="http://example.org/onto/class/google_compute_instance_template"/>
    <rdfs:range rdf:resource="http://www.w3.org/2001/XMLSchema#string"/>
  </owl:DatatypeProperty>
  <owl:DatatypeProperty rdf:about="http://example.org/onto/prop/google_compute_instance_template_mode">
    <rdfs:label>mode</rdfs:label>
    <rdfs:comment>The mode in which to attach this disk, either READ_WRITE or READ_ONLY. If you are attaching or creating a boot disk, this must read-write mode.</rdfs:comment>
    <rdfs:domain rdf:resource="http://example.org/onto/class/google_compute_instance_template"/>
    <rdfs:range rdf:resource="http://www.w3.org/2001/XMLSchema#string"/>
  </owl:DatatypeProperty>
  <owl:DatatypeProperty rdf:about="http://example.org/onto/prop/google_compute_instance_template_provisioned_iops">
    <rdfs:label>provisioned_iops</rdfs:label>
    <rdfs:comment>Indicates how many IOPS to provision for the disk. This sets the number of I/O operations per second that the disk can handle. For more details, see the [Extreme persistent disk documentation](https://cloud.google.com/compute/docs/disks/extreme-persistent-disk) or the [Hyperdisk documentation](https://cloud.google.com/compute/docs/disks/hyperdisks) depending on the selected disk_type.</rdfs:comment>
    <rdfs:domain rdf:resource="http://example.org/onto/class/google_compute_instance_template"/>
    <rdfs:range rdf:resource="http://www.w3.org/2001/XMLSchema#string"/>
  </owl:DatatypeProperty>
  <owl:DatatypeProperty rdf:about="http://example.org/onto/prop/google_compute_instance_template_provisioned_throughput">
    <rdfs:label>provisioned_throughput</rdfs:label>
    <rdfs:comment>Indicates how much throughput to provision for the disk, in MB/s. This sets the amount of data that can be read or written from the disk per second. Values must greater than or equal to 1. For more details, see the [Hyperdisk documentation](https://cloud.google.com/compute/docs/disks/hyperdisks).</rdfs:comment>
    <rdfs:domain rdf:resource="http://example.org/onto/class/google_compute_instance_template"/>
    <rdfs:range rdf:resource="http://www.w3.org/2001/XMLSchema#string"/>
  </owl:DatatypeProperty>
  <owl:DatatypeProperty rdf:about="http://example.org/onto/prop/google_compute_instance_template_resource_manager_tags">
    <rdfs:label>resource_manager_tags</rdfs:label>
    <rdfs:comment>A map of resource manager tags. Resource manager tag keys and values have the same definition as resource manager tags. Keys must be in the format tagKeys/{tag_key_id}, and values are in the format tagValues/456. The field is ignored (both PUT & PATCH) when empty.</rdfs:comment>
    <rdfs:domain rdf:resource="http://example.org/onto/class/google_compute_instance_template"/>
    <rdfs:range rdf:resource="http://www.w3.org/2001/XMLSchema#string"/>
  </owl:DatatypeProperty>
  <owl:DatatypeProperty rdf:about="http://example.org/onto/prop/google_compute_instance_template_resource_policies">
    <rdfs:label>resource_policies</rdfs:label>
    <rdfs:comment>A list (short name or id) of resource policies to attach to this disk. Currently a max of 1 resource policy is supported.</rdfs:comment>
    <rdfs:domain rdf:resource="http://example.org/onto/class/google_compute_instance_template"/>
    <rdfs:range rdf:resource="http://www.w3.org/2001/XMLSchema#string"/>
  </owl:DatatypeProperty>
  <owl:DatatypeProperty rdf:about="http://example.org/onto/prop/google_compute_instance_template_source">
    <rdfs:label>source</rdfs:label>
    <rdfs:comment>The name (not self_link) of the disk (such as those managed by google_compute_disk) to attach. ~> Note: Either source or source_image is required when creating a new instance except for when creating a local SSD.</rdfs:comment>
    <rdfs:domain rdf:resource="http://example.org/onto/class/google_compute_instance_template"/>
    <rdfs:range rdf:resource="http://www.w3.org/2001/XMLSchema#string"/>
  </owl:DatatypeProperty>
  <owl:DatatypeProperty rdf:about="http://example.org/onto/prop/google_compute_instance_template_source_image">
    <rdfs:label>source_image</rdfs:label>
    <rdfs:comment>The image from which to initialize this disk. This can be one of: the image's self_link, projects/{project}/global/images/{image}, projects/{project}/global/images/family/{family}, global/images/{image}, global/images/family/{family}, family/{family}, {project}/{family}, {project}/{image}, {family}, or {image}. ~> Note: Either source or source_image is required when creating a new instance except for when creating a local SSD.</rdfs:comment>
    <rdfs:domain rdf:resource="http://example.org/onto/class/google_compute_instance_template"/>
    <rdfs:range rdf:resource="http://www.w3.org/2001/XMLSchema#string"/>
  </owl:DatatypeProperty>
  <owl:DatatypeProperty rdf:about="http://example.org/onto/prop/google_compute_instance_template_source_snapshot">
    <rdfs:label>source_snapshot</rdfs:label>
    <rdfs:comment>The source snapshot to create this disk. When creating
a new instance, one of initializeParams.sourceSnapshot,
initializeParams.sourceImage, or disks.source is
required except for local SSD.</rdfs:comment>
    <rdfs:domain rdf:resource="http://example.org/onto/class/google_compute_instance_template"/>
    <rdfs:range rdf:resource="http://www.w3.org/2001/XMLSchema#string"/>
  </owl:DatatypeProperty>
  <owl:DatatypeProperty rdf:about="http://example.org/onto/prop/google_compute_instance_template_type">
    <rdfs:label>type</rdfs:label>
    <rdfs:comment>The type of Google Compute Engine disk, can be either "SCRATCH" or "PERSISTENT".</rdfs:comment>
    <rdfs:domain rdf:resource="http://example.org/onto/class/google_compute_instance_template"/>
    <rdfs:range rdf:resource="http://www.w3.org/2001/XMLSchema#string"/>
  </owl:DatatypeProperty>
  <owl:DatatypeProperty rdf:about="http://example.org/onto/prop/google_compute_instance_template_kms_key_self_link">
    <rdfs:label>kms_key_self_link</rdfs:label>
    <rdfs:comment>The self link of the encryption key that is stored in Google Cloud KMS.</rdfs:comment>
    <rdfs:domain rdf:resource="http://example.org/onto/class/google_compute_instance_template"/>
    <rdfs:range rdf:resource="http://www.w3.org/2001/XMLSchema#string"/>
  </owl:DatatypeProperty>
  <owl:DatatypeProperty rdf:about="http://example.org/onto/prop/google_compute_instance_template_kms_key_service_account">
    <rdfs:label>kms_key_service_account</rdfs:label>
    <rdfs:comment>The service account being used for the encryption request for the given KMS key. If absent, the Compute Engine default service account is used.</rdfs:comment>
    <rdfs:domain rdf:resource="http://example.org/onto/class/google_compute_instance_template"/>
    <rdfs:range rdf:resource="http://www.w3.org/2001/XMLSchema#string"/>
  </owl:DatatypeProperty>
  <owl:DatatypeProperty rdf:about="http://example.org/onto/prop/google_compute_instance_template_kms_key_self_link">
    <rdfs:label>kms_key_self_link</rdfs:label>
    <rdfs:comment>The self link of the encryption key that is stored in
Google Cloud KMS. Only one of kms_key_self_link, rsa_encrypted_key and raw_key may be set.</rdfs:comment>
    <rdfs:domain rdf:resource="http://example.org/onto/class/google_compute_instance_template"/>
    <rdfs:range rdf:resource="http://www.w3.org/2001/XMLSchema#string"/>
  </owl:DatatypeProperty>
  <owl:DatatypeProperty rdf:about="http://example.org/onto/prop/google_compute_instance_template_kms_key_service_account">
    <rdfs:label>kms_key_service_account</rdfs:label>
    <rdfs:comment>The service account being used for the encryption
request for the given KMS key. If absent, the Compute
Engine default service account is used.</rdfs:comment>
    <rdfs:domain rdf:resource="http://example.org/onto/class/google_compute_instance_template"/>
    <rdfs:range rdf:resource="http://www.w3.org/2001/XMLSchema#string"/>
  </owl:DatatypeProperty>
  <owl:DatatypeProperty rdf:about="http://example.org/onto/prop/google_compute_instance_template_raw_key">
    <rdfs:label>raw_key</rdfs:label>
    <rdfs:comment>Specifies a 256-bit customer-supplied encryption key, encoded in RFC 4648 base64 to either encrypt or decrypt this resource. Only one of kms_key_self_link, rsa_encrypted_key and raw_key may be set.</rdfs:comment>
    <rdfs:domain rdf:resource="http://example.org/onto/class/google_compute_instance_template"/>
    <rdfs:range rdf:resource="http://www.w3.org/2001/XMLSchema#string"/>
  </owl:DatatypeProperty>
  <owl:DatatypeProperty rdf:about="http://example.org/onto/prop/google_compute_instance_template_rsa_encrypted_key">
    <rdfs:label>rsa_encrypted_key</rdfs:label>
    <rdfs:comment>Specifies an RFC 4648 base64 encoded, RSA-wrapped 2048-bit customer-supplied encryption key to either encrypt or decrypt this resource. Only one of kms_key_self_link, rsa_encrypted_key and raw_key may be set.</rdfs:comment>
    <rdfs:domain rdf:resource="http://example.org/onto/class/google_compute_instance_template"/>
    <rdfs:range rdf:resource="http://www.w3.org/2001/XMLSchema#string"/>
  </owl:DatatypeProperty>
  <owl:DatatypeProperty rdf:about="http://example.org/onto/prop/google_compute_instance_template_kms_key_self_link">
    <rdfs:label>kms_key_self_link</rdfs:label>
    <rdfs:comment>The self link of the encryption key that is stored in
Google Cloud KMS. Only one of kms_key_self_link, rsa_encrypted_key and raw_key may be set.</rdfs:comment>
    <rdfs:domain rdf:resource="http://example.org/onto/class/google_compute_instance_template"/>
    <rdfs:range rdf:resource="http://www.w3.org/2001/XMLSchema#string"/>
  </owl:DatatypeProperty>
  <owl:DatatypeProperty rdf:about="http://example.org/onto/prop/google_compute_instance_template_kms_key_service_account">
    <rdfs:label>kms_key_service_account</rdfs:label>
    <rdfs:comment>The service account being used for the encryption
request for the given KMS key. If absent, the Compute
Engine default service account is used.</rdfs:comment>
    <rdfs:domain rdf:resource="http://example.org/onto/class/google_compute_instance_template"/>
    <rdfs:range rdf:resource="http://www.w3.org/2001/XMLSchema#string"/>
  </owl:DatatypeProperty>
  <owl:DatatypeProperty rdf:about="http://example.org/onto/prop/google_compute_instance_template_raw_key">
    <rdfs:label>raw_key</rdfs:label>
    <rdfs:comment>Specifies a 256-bit customer-supplied encryption key, encoded in RFC 4648 base64 to either encrypt or decrypt this resource. Only one of kms_key_self_link, rsa_encrypted_key and raw_key may be set.</rdfs:comment>
    <rdfs:domain rdf:resource="http://example.org/onto/class/google_compute_instance_template"/>
    <rdfs:range rdf:resource="http://www.w3.org/2001/XMLSchema#string"/>
  </owl:DatatypeProperty>
  <owl:DatatypeProperty rdf:about="http://example.org/onto/prop/google_compute_instance_template_rsa_encrypted_key">
    <rdfs:label>rsa_encrypted_key</rdfs:label>
    <rdfs:comment>Specifies an RFC 4648 base64 encoded, RSA-wrapped 2048-bit customer-supplied encryption key to either encrypt or decrypt this resource. Only one of kms_key_self_link, rsa_encrypted_key and raw_key may be set.</rdfs:comment>
    <rdfs:domain rdf:resource="http://example.org/onto/class/google_compute_instance_template"/>
    <rdfs:range rdf:resource="http://www.w3.org/2001/XMLSchema#string"/>
  </owl:DatatypeProperty>
  <owl:DatatypeProperty rdf:about="http://example.org/onto/prop/google_compute_instance_template_count">
    <rdfs:label>count</rdfs:label>
    <rdfs:comment>The number of the guest accelerator cards exposed to this instance.</rdfs:comment>
    <rdfs:domain rdf:resource="http://example.org/onto/class/google_compute_instance_template"/>
    <rdfs:range rdf:resource="http://www.w3.org/2001/XMLSchema#string"/>
  </owl:DatatypeProperty>
  <owl:DatatypeProperty rdf:about="http://example.org/onto/prop/google_compute_instance_template_type">
    <rdfs:label>type</rdfs:label>
    <rdfs:comment>The accelerator type resource to expose to this instance. E.g. nvidia-tesla-k80.</rdfs:comment>
    <rdfs:domain rdf:resource="http://example.org/onto/class/google_compute_instance_template"/>
    <rdfs:range rdf:resource="http://www.w3.org/2001/XMLSchema#string"/>
  </owl:DatatypeProperty>
  <owl:DatatypeProperty rdf:about="http://example.org/onto/prop/google_compute_instance_template_internal_ipv6_prefix_length">
    <rdfs:label>internal_ipv6_prefix_length</rdfs:label>
    <rdfs:comment>The prefix length of the primary internal IPv6 range.</rdfs:comment>
    <rdfs:domain rdf:resource="http://example.org/onto/class/google_compute_instance_template"/>
    <rdfs:range rdf:resource="http://www.w3.org/2001/XMLSchema#string"/>
  </owl:DatatypeProperty>
  <owl:DatatypeProperty rdf:about="http://example.org/onto/prop/google_compute_instance_template_ipv6_access_type">
    <rdfs:label>ipv6_access_type</rdfs:label>
    <rdfs:comment>One of EXTERNAL, INTERNAL to indicate whether the IP can be accessed from the Internet. This field is always inherited from its subnetwork.</rdfs:comment>
    <rdfs:domain rdf:resource="http://example.org/onto/class/google_compute_instance_template"/>
    <rdfs:range rdf:resource="http://www.w3.org/2001/XMLSchema#string"/>
  </owl:DatatypeProperty>
  <owl:DatatypeProperty rdf:about="http://example.org/onto/prop/google_compute_instance_template_ipv6_address">
    <rdfs:label>ipv6_address</rdfs:label>
    <rdfs:comment>An IPv6 internal network address for this network interface. If not specified, Google Cloud will automatically assign an internal IPv6 address from the instance's subnetwork.</rdfs:comment>
    <rdfs:domain rdf:resource="http://example.org/onto/class/google_compute_instance_template"/>
    <rdfs:range rdf:resource="http://www.w3.org/2001/XMLSchema#string"/>
  </owl:DatatypeProperty>
  <owl:DatatypeProperty rdf:about="http://example.org/onto/prop/google_compute_instance_template_name">
    <rdfs:label>name</rdfs:label>
    <rdfs:comment>The name of the network_interface.</rdfs:comment>
    <rdfs:domain rdf:resource="http://example.org/onto/class/google_compute_instance_template"/>
    <rdfs:range rdf:resource="http://www.w3.org/2001/XMLSchema#string"/>
  </owl:DatatypeProperty>
  <owl:DatatypeProperty rdf:about="http://example.org/onto/prop/google_compute_instance_template_network">
    <rdfs:label>network</rdfs:label>
    <rdfs:comment>The name or self_link of the network to attach this interface to. Use network attribute for Legacy or Auto subnetted networks and subnetwork for custom subnetted networks.</rdfs:comment>
    <rdfs:domain rdf:resource="http://example.org/onto/class/google_compute_instance_template"/>
    <rdfs:range rdf:resource="http://www.w3.org/2001/XMLSchema#string"/>
  </owl:DatatypeProperty>
  <owl:DatatypeProperty rdf:about="http://example.org/onto/prop/google_compute_instance_template_network_ip">
    <rdfs:label>network_ip</rdfs:label>
    <rdfs:comment>The private IP address to assign to the instance. If empty, the address will be automatically assigned.</rdfs:comment>
    <rdfs:domain rdf:resource="http://example.org/onto/class/google_compute_instance_template"/>
    <rdfs:range rdf:resource="http://www.w3.org/2001/XMLSchema#string"/>
  </owl:DatatypeProperty>
  <owl:DatatypeProperty rdf:about="http://example.org/onto/prop/google_compute_instance_template_nic_type">
    <rdfs:label>nic_type</rdfs:label>
    <rdfs:comment>The type of vNIC to be used on this interface. Possible values:GVNIC, VIRTIO_NET, MRDMA, and IRDMA</rdfs:comment>
    <rdfs:domain rdf:resource="http://example.org/onto/class/google_compute_instance_template"/>
    <rdfs:range rdf:resource="http://www.w3.org/2001/XMLSchema#string"/>
  </owl:DatatypeProperty>
  <owl:DatatypeProperty rdf:about="http://example.org/onto/prop/google_compute_instance_template_queue_count">
    <rdfs:label>queue_count</rdfs:label>
    <rdfs:comment>The networking queue count that's specified by users for the network interface. Both Rx and Tx queues will be set to this number. It will be empty if not specified.</rdfs:comment>
    <rdfs:domain rdf:resource="http://example.org/onto/class/google_compute_instance_template"/>
    <rdfs:range rdf:resource="http://www.w3.org/2001/XMLSchema#string"/>
  </owl:DatatypeProperty>
  <owl:DatatypeProperty rdf:about="http://example.org/onto/prop/google_compute_instance_template_stack_type">
    <rdfs:label>stack_type</rdfs:label>
    <rdfs:comment>The stack type for this network interface to identify whether the IPv6 feature is enabled or not. If not specified, IPV4_ONLY will be used.</rdfs:comment>
    <rdfs:domain rdf:resource="http://example.org/onto/class/google_compute_instance_template"/>
    <rdfs:range rdf:resource="http://www.w3.org/2001/XMLSchema#string"/>
  </owl:DatatypeProperty>
  <owl:DatatypeProperty rdf:about="http://example.org/onto/prop/google_compute_instance_template_subnetwork">
    <rdfs:label>subnetwork</rdfs:label>
    <rdfs:comment>The name of the subnetwork to attach this interface to. The subnetwork must exist in the same region this instance will be created in. Either network or subnetwork must be provided.</rdfs:comment>
    <rdfs:domain rdf:resource="http://example.org/onto/class/google_compute_instance_template"/>
    <rdfs:range rdf:resource="http://www.w3.org/2001/XMLSchema#string"/>
  </owl:DatatypeProperty>
  <owl:DatatypeProperty rdf:about="http://example.org/onto/prop/google_compute_instance_template_subnetwork_project">
    <rdfs:label>subnetwork_project</rdfs:label>
    <rdfs:comment>The ID of the project in which the subnetwork belongs. If it is not provided, the provider project is used.</rdfs:comment>
    <rdfs:domain rdf:resource="http://example.org/onto/class/google_compute_instance_template"/>
    <rdfs:range rdf:resource="http://www.w3.org/2001/XMLSchema#string"/>
  </owl:DatatypeProperty>
  <owl:DatatypeProperty rdf:about="http://example.org/onto/prop/google_compute_instance_template_nat_ip">
    <rdfs:label>nat_ip</rdfs:label>
    <rdfs:comment>The IP address that will be 1:1 mapped to the instance's network ip. If not given, one will be generated.</rdfs:comment>
    <rdfs:domain rdf:resource="http://example.org/onto/class/google_compute_instance_template"/>
    <rdfs:range rdf:resource="http://www.w3.org/2001/XMLSchema#string"/>
  </owl:DatatypeProperty>
  <owl:DatatypeProperty rdf:about="http://example.org/onto/prop/google_compute_instance_template_network_tier">
    <rdfs:label>network_tier</rdfs:label>
    <rdfs:comment>The networking tier used for configuring this instance template. This field can take the following values: PREMIUM, STANDARD, FIXED_STANDARD. If this field is not specified, it is assumed to be PREMIUM.</rdfs:comment>
    <rdfs:domain rdf:resource="http://example.org/onto/class/google_compute_instance_template"/>
    <rdfs:range rdf:resource="http://www.w3.org/2001/XMLSchema#string"/>
  </owl:DatatypeProperty>
  <owl:DatatypeProperty rdf:about="http://example.org/onto/prop/google_compute_instance_template_public_ptr_domain_name">
    <rdfs:label>public_ptr_domain_name</rdfs:label>
    <rdfs:comment>The DNS domain name for the public PTR record.The DNS domain name for the public PTR record.</rdfs:comment>
    <rdfs:domain rdf:resource="http://example.org/onto/class/google_compute_instance_template"/>
    <rdfs:range rdf:resource="http://www.w3.org/2001/XMLSchema#string"/>
  </owl:DatatypeProperty>
  <owl:DatatypeProperty rdf:about="http://example.org/onto/prop/google_compute_instance_template_ip_cidr_range">
    <rdfs:label>ip_cidr_range</rdfs:label>
    <rdfs:comment>The IP CIDR range represented by this alias IP range. This IP CIDR range must belong to the specified subnetwork and cannot contain IP addresses reserved by system or used by other network interfaces. At the time of writing only a netmask (e.g. /24) may be supplied, with a CIDR format resulting in an API error.</rdfs:comment>
    <rdfs:domain rdf:resource="http://example.org/onto/class/google_compute_instance_template"/>
    <rdfs:range rdf:resource="http://www.w3.org/2001/XMLSchema#string"/>
  </owl:DatatypeProperty>
  <owl:DatatypeProperty rdf:about="http://example.org/onto/prop/google_compute_instance_template_subnetwork_range_name">
    <rdfs:label>subnetwork_range_name</rdfs:label>
    <rdfs:comment>The subnetwork secondary range name specifying the secondary range from which to allocate the IP CIDR range for this alias IP range. If left unspecified, the primary range of the subnetwork will be used.</rdfs:comment>
    <rdfs:domain rdf:resource="http://example.org/onto/class/google_compute_instance_template"/>
    <rdfs:range rdf:resource="http://www.w3.org/2001/XMLSchema#string"/>
  </owl:DatatypeProperty>
  <owl:DatatypeProperty rdf:about="http://example.org/onto/prop/google_compute_instance_template_external_ipv6">
    <rdfs:label>external_ipv6</rdfs:label>
    <rdfs:comment>The first IPv6 address of the external IPv6 range associated with this instance, prefix length is stored in externalIpv6PrefixLength in ipv6AccessConfig. The field is output only, an IPv6 address from a subnetwork associated with the instance will be allocated dynamically.</rdfs:comment>
    <rdfs:domain rdf:resource="http://example.org/onto/class/google_compute_instance_template"/>
    <rdfs:range rdf:resource="http://www.w3.org/2001/XMLSchema#string"/>
  </owl:DatatypeProperty>
  <owl:DatatypeProperty rdf:about="http://example.org/onto/prop/google_compute_instance_template_external_ipv6_prefix_length">
    <rdfs:label>external_ipv6_prefix_length</rdfs:label>
    <rdfs:comment>The prefix length of the external IPv6 range.</rdfs:comment>
    <rdfs:domain rdf:resource="http://example.org/onto/class/google_compute_instance_template"/>
    <rdfs:range rdf:resource="http://www.w3.org/2001/XMLSchema#string"/>
  </owl:DatatypeProperty>
  <owl:DatatypeProperty rdf:about="http://example.org/onto/prop/google_compute_instance_template_name">
    <rdfs:label>name</rdfs:label>
    <rdfs:comment>The name of this access configuration.</rdfs:comment>
    <rdfs:domain rdf:resource="http://example.org/onto/class/google_compute_instance_template"/>
    <rdfs:range rdf:resource="http://www.w3.org/2001/XMLSchema#string"/>
  </owl:DatatypeProperty>
  <owl:DatatypeProperty rdf:about="http://example.org/onto/prop/google_compute_instance_template_network_tier">
    <rdfs:label>network_tier</rdfs:label>
    <rdfs:comment>The service-level to be provided for IPv6 traffic when the subnet has an external subnet. Only PREMIUM tier is valid for IPv6</rdfs:comment>
    <rdfs:domain rdf:resource="http://example.org/onto/class/google_compute_instance_template"/>
    <rdfs:range rdf:resource="http://www.w3.org/2001/XMLSchema#string"/>
  </owl:DatatypeProperty>
  <owl:DatatypeProperty rdf:about="http://example.org/onto/prop/google_compute_instance_template_public_ptr_domain_name">
    <rdfs:label>public_ptr_domain_name</rdfs:label>
    <rdfs:comment>The domain name to be used when creating DNSv6 records for the external IPv6 ranges.</rdfs:comment>
    <rdfs:domain rdf:resource="http://example.org/onto/class/google_compute_instance_template"/>
    <rdfs:range rdf:resource="http://www.w3.org/2001/XMLSchema#string"/>
  </owl:DatatypeProperty>
  <owl:DatatypeProperty rdf:about="http://example.org/onto/prop/google_compute_instance_template_total_egress_bandwidth_tier">
    <rdfs:label>total_egress_bandwidth_tier</rdfs:label>
    <rdfs:comment>The egress bandwidth tier to enable. Possible values:TIER_1, DEFAULT</rdfs:comment>
    <rdfs:domain rdf:resource="http://example.org/onto/class/google_compute_instance_template"/>
    <rdfs:range rdf:resource="http://www.w3.org/2001/XMLSchema#string"/>
  </owl:DatatypeProperty>
  <owl:DatatypeProperty rdf:about="http://example.org/onto/prop/google_compute_instance_template_type">
    <rdfs:label>type</rdfs:label>
    <rdfs:comment>The type of reservation from which this instance can consume resources.</rdfs:comment>
    <rdfs:domain rdf:resource="http://example.org/onto/class/google_compute_instance_template"/>
    <rdfs:range rdf:resource="http://www.w3.org/2001/XMLSchema#string"/>
  </owl:DatatypeProperty>
  <owl:DatatypeProperty rdf:about="http://example.org/onto/prop/google_compute_instance_template_key">
    <rdfs:label>key</rdfs:label>
    <rdfs:comment>Corresponds to the label key of a reservation resource. To target a SPECIFIC_RESERVATION by name, specify compute.googleapis.com/reservation-name as the key and specify the name of your reservation as the only value.</rdfs:comment>
    <rdfs:domain rdf:resource="http://example.org/onto/class/google_compute_instance_template"/>
    <rdfs:range rdf:resource="http://www.w3.org/2001/XMLSchema#string"/>
  </owl:DatatypeProperty>
  <owl:DatatypeProperty rdf:about="http://example.org/onto/prop/google_compute_instance_template_values">
    <rdfs:label>values</rdfs:label>
    <rdfs:comment>Corresponds to the label values of a reservation resource.</rdfs:comment>
    <rdfs:domain rdf:resource="http://example.org/onto/class/google_compute_instance_template"/>
    <rdfs:range rdf:resource="http://www.w3.org/2001/XMLSchema#string"/>
  </owl:DatatypeProperty>
  <owl:DatatypeProperty rdf:about="http://example.org/onto/prop/google_compute_instance_template_automatic_restart">
    <rdfs:label>automatic_restart</rdfs:label>
    <rdfs:comment>Specifies whether the instance should be automatically restarted if it is terminated by Compute Engine (not terminated by a user). This defaults to true.</rdfs:comment>
    <rdfs:domain rdf:resource="http://example.org/onto/class/google_compute_instance_template"/>
    <rdfs:range rdf:resource="http://www.w3.org/2001/XMLSchema#string"/>
  </owl:DatatypeProperty>
  <owl:DatatypeProperty rdf:about="http://example.org/onto/prop/google_compute_instance_template_availability_domain">
    <rdfs:label>availability_domain</rdfs:label>
    <rdfs:comment>Specifies the availability domain, which this instance should be scheduled on.</rdfs:comment>
    <rdfs:domain rdf:resource="http://example.org/onto/class/google_compute_instance_template"/>
    <rdfs:range rdf:resource="http://www.w3.org/2001/XMLSchema#string"/>
  </owl:DatatypeProperty>
  <owl:DatatypeProperty rdf:about="http://example.org/onto/prop/google_compute_instance_template_instance_termination_action">
    <rdfs:label>instance_termination_action</rdfs:label>
    <rdfs:comment>Specifies the action GCE should take when SPOT VM is preempted.</rdfs:comment>
    <rdfs:domain rdf:resource="http://example.org/onto/class/google_compute_instance_template"/>
    <rdfs:range rdf:resource="http://www.w3.org/2001/XMLSchema#string"/>
  </owl:DatatypeProperty>
  <owl:DatatypeProperty rdf:about="http://example.org/onto/prop/google_compute_instance_template_min_node_cpus">
    <rdfs:label>min_node_cpus</rdfs:label>
    <rdfs:comment>Minimum number of cpus for the instance.</rdfs:comment>
    <rdfs:domain rdf:resource="http://example.org/onto/class/google_compute_instance_template"/>
    <rdfs:range rdf:resource="http://www.w3.org/2001/XMLSchema#string"/>
  </owl:DatatypeProperty>
  <owl:DatatypeProperty rdf:about="http://example.org/onto/prop/google_compute_instance_template_on_host_maintenance">
    <rdfs:label>on_host_maintenance</rdfs:label>
    <rdfs:comment>Defines the maintenance behavior for this instance.</rdfs:comment>
    <rdfs:domain rdf:resource="http://example.org/onto/class/google_compute_instance_template"/>
    <rdfs:range rdf:resource="http://www.w3.org/2001/XMLSchema#string"/>
  </owl:DatatypeProperty>
  <owl:DatatypeProperty rdf:about="http://example.org/onto/prop/google_compute_instance_template_preemptible">
    <rdfs:label>preemptible</rdfs:label>
    <rdfs:comment>Allows instance to be preempted. This defaults to false.</rdfs:comment>
    <rdfs:domain rdf:resource="http://example.org/onto/class/google_compute_instance_template"/>
    <rdfs:range rdf:resource="http://www.w3.org/2001/XMLSchema#string"/>
  </owl:DatatypeProperty>
  <owl:DatatypeProperty rdf:about="http://example.org/onto/prop/google_compute_instance_template_provisioning_model">
    <rdfs:label>provisioning_model</rdfs:label>
    <rdfs:comment>Whether the instance is spot. If this is set as SPOT.</rdfs:comment>
    <rdfs:domain rdf:resource="http://example.org/onto/class/google_compute_instance_template"/>
    <rdfs:range rdf:resource="http://www.w3.org/2001/XMLSchema#string"/>
  </owl:DatatypeProperty>
  <owl:DatatypeProperty rdf:about="http://example.org/onto/prop/google_compute_instance_template_termination_time">
    <rdfs:label>termination_time</rdfs:label>
    <rdfs:comment>Specifies the timestamp, when the instance will be terminated,
in RFC3339 text format. If specified, the instance termination action
will be performed at the termination time.</rdfs:comment>
    <rdfs:domain rdf:resource="http://example.org/onto/class/google_compute_instance_template"/>
    <rdfs:range rdf:resource="http://www.w3.org/2001/XMLSchema#string"/>
  </owl:DatatypeProperty>
  <owl:DatatypeProperty rdf:about="http://example.org/onto/prop/google_compute_instance_template_nanos">
    <rdfs:label>nanos</rdfs:label>
    <rdfs:comment>Span of time that's a fraction of a second at nanosecond
resolution. Durations less than one second are represented
with a 0 seconds field and a positive nanos field. Must
be from 0 to 999,999,999 inclusive.</rdfs:comment>
    <rdfs:domain rdf:resource="http://example.org/onto/class/google_compute_instance_template"/>
    <rdfs:range rdf:resource="http://www.w3.org/2001/XMLSchema#string"/>
  </owl:DatatypeProperty>
  <owl:DatatypeProperty rdf:about="http://example.org/onto/prop/google_compute_instance_template_seconds">
    <rdfs:label>seconds</rdfs:label>
    <rdfs:comment>Span of time at a resolution of a second.
Must be from 0 to 315,576,000,000 inclusive.</rdfs:comment>
    <rdfs:domain rdf:resource="http://example.org/onto/class/google_compute_instance_template"/>
    <rdfs:range rdf:resource="http://www.w3.org/2001/XMLSchema#string"/>
  </owl:DatatypeProperty>
  <owl:DatatypeProperty rdf:about="http://example.org/onto/prop/google_compute_instance_template_nanos">
    <rdfs:label>nanos</rdfs:label>
    <rdfs:comment>Span of time that's a fraction of a second at nanosecond
resolution. Durations less than one second are represented
with a 0 seconds field and a positive nanos field. Must
be from 0 to 999,999,999 inclusive.</rdfs:comment>
    <rdfs:domain rdf:resource="http://example.org/onto/class/google_compute_instance_template"/>
    <rdfs:range rdf:resource="http://www.w3.org/2001/XMLSchema#string"/>
  </owl:DatatypeProperty>
  <owl:DatatypeProperty rdf:about="http://example.org/onto/prop/google_compute_instance_template_seconds">
    <rdfs:label>seconds</rdfs:label>
    <rdfs:comment>Span of time at a resolution of a second.
Must be from 0 to 315,576,000,000 inclusive.</rdfs:comment>
    <rdfs:domain rdf:resource="http://example.org/onto/class/google_compute_instance_template"/>
    <rdfs:range rdf:resource="http://www.w3.org/2001/XMLSchema#string"/>
  </owl:DatatypeProperty>
  <owl:DatatypeProperty rdf:about="http://example.org/onto/prop/google_compute_instance_template_key">
    <rdfs:label>key</rdfs:label>
    <rdfs:domain rdf:resource="http://example.org/onto/class/google_compute_instance_template"/>
    <rdfs:range rdf:resource="http://www.w3.org/2001/XMLSchema#string"/>
  </owl:DatatypeProperty>
  <owl:DatatypeProperty rdf:about="http://example.org/onto/prop/google_compute_instance_template_operator">
    <rdfs:label>operator</rdfs:label>
    <rdfs:domain rdf:resource="http://example.org/onto/class/google_compute_instance_template"/>
    <rdfs:range rdf:resource="http://www.w3.org/2001/XMLSchema#string"/>
  </owl:DatatypeProperty>
  <owl:DatatypeProperty rdf:about="http://example.org/onto/prop/google_compute_instance_template_values">
    <rdfs:label>values</rdfs:label>
    <rdfs:domain rdf:resource="http://example.org/onto/class/google_compute_instance_template"/>
    <rdfs:range rdf:resource="http://www.w3.org/2001/XMLSchema#string"/>
  </owl:DatatypeProperty>
  <owl:DatatypeProperty rdf:about="http://example.org/onto/prop/google_compute_instance_template_discard_local_ssd">
    <rdfs:label>discard_local_ssd</rdfs:label>
    <rdfs:comment>If true, the contents of any attached Local SSD disks will be discarded.</rdfs:comment>
    <rdfs:domain rdf:resource="http://example.org/onto/class/google_compute_instance_template"/>
    <rdfs:range rdf:resource="http://www.w3.org/2001/XMLSchema#string"/>
  </owl:DatatypeProperty>
  <owl:DatatypeProperty rdf:about="http://example.org/onto/prop/google_compute_instance_template_email">
    <rdfs:label>email</rdfs:label>
    <rdfs:comment>The service account e-mail address. If not given, the default Google Compute Engine service account is used.</rdfs:comment>
    <rdfs:domain rdf:resource="http://example.org/onto/class/google_compute_instance_template"/>
    <rdfs:range rdf:resource="http://www.w3.org/2001/XMLSchema#string"/>
  </owl:DatatypeProperty>
  <owl:DatatypeProperty rdf:about="http://example.org/onto/prop/google_compute_instance_template_scopes">
    <rdfs:label>scopes</rdfs:label>
    <rdfs:comment>A list of service scopes. Both OAuth2 URLs and gcloud short names are supported. To allow full access to all Cloud APIs, use the cloud-platform scope.</rdfs:comment>
    <rdfs:domain rdf:resource="http://example.org/onto/class/google_compute_instance_template"/>
    <rdfs:range rdf:resource="http://www.w3.org/2001/XMLSchema#string"/>
  </owl:DatatypeProperty>
  <owl:DatatypeProperty rdf:about="http://example.org/onto/prop/google_compute_instance_template_enable_integrity_monitoring">
    <rdfs:label>enable_integrity_monitoring</rdfs:label>
    <rdfs:comment>Compare the most recent boot measurements to the integrity policy baseline and return a pair of pass/fail results depending on whether they match or not. Defaults to true.</rdfs:comment>
    <rdfs:domain rdf:resource="http://example.org/onto/class/google_compute_instance_template"/>
    <rdfs:range rdf:resource="http://www.w3.org/2001/XMLSchema#string"/>
  </owl:DatatypeProperty>
  <owl:DatatypeProperty rdf:about="http://example.org/onto/prop/google_compute_instance_template_enable_secure_boot">
    <rdfs:label>enable_secure_boot</rdfs:label>
    <rdfs:comment>Verify the digital signature of all boot components, and halt the boot process if signature verification fails. Defaults to false.</rdfs:comment>
    <rdfs:domain rdf:resource="http://example.org/onto/class/google_compute_instance_template"/>
    <rdfs:range rdf:resource="http://www.w3.org/2001/XMLSchema#string"/>
  </owl:DatatypeProperty>
  <owl:DatatypeProperty rdf:about="http://example.org/onto/prop/google_compute_instance_template_enable_vtpm">
    <rdfs:label>enable_vtpm</rdfs:label>
    <rdfs:comment>Use a virtualized trusted platform module, which is a specialized computer chip you can use to encrypt objects like keys and certificates. Defaults to true.</rdfs:comment>
    <rdfs:domain rdf:resource="http://example.org/onto/class/google_compute_instance_template"/>
    <rdfs:range rdf:resource="http://www.w3.org/2001/XMLSchema#string"/>
  </owl:DatatypeProperty>
  <owl:DatatypeProperty rdf:about="http://example.org/onto/prop/google_compute_instance_template_create">
    <rdfs:label>create</rdfs:label>
    <rdfs:domain rdf:resource="http://example.org/onto/class/google_compute_instance_template"/>
    <rdfs:range rdf:resource="http://www.w3.org/2001/XMLSchema#string"/>
  </owl:DatatypeProperty>
  <owl:DatatypeProperty rdf:about="http://example.org/onto/prop/google_compute_instance_template_delete">
    <rdfs:label>delete</rdfs:label>
    <rdfs:domain rdf:resource="http://example.org/onto/class/google_compute_instance_template"/>
    <rdfs:range rdf:resource="http://www.w3.org/2001/XMLSchema#string"/>
  </owl:DatatypeProperty>
</rdf:RDF>
