<?xml version="1.0" encoding="UTF-8"?>
<rdf:RDF
  xmlns:rdf="http://www.w3.org/1999/02/22-rdf-syntax-ns#"
  xmlns:rdfs="http://www.w3.org/2000/01/rdf-schema#"
  xmlns:owl="http://www.w3.org/2002/07/owl#"
  xmlns:xsd="http://www.w3.org/2001/XMLSchema#"
  xml:base="http://example.org/onto/">
  <owl:Class rdf:about="http://example.org/onto/class/google_data_loss_prevention_deidentify_template">
    <rdfs:label>google_data_loss_prevention_deidentify_template</rdfs:label>
    <rdfs:comment>#
#     ***     AUTO GENERATED CODE    ***    Type: MMv1     ***
#
# ----------------------------------------------------------------------------
#
#     This code is generated by Magic Modules using the following:
#
#     Configuration: https:#github.com/GoogleCloudPlatform/magic-modules/tree/main/mmv1/products/dlp/DeidentifyTemplate.yaml
#     Template:      https:#github.com/GoogleCloudPlatform/magic-modules/tree/main/mmv1/templates/terraform/resource.html.markdown.tmpl
#
#     DO NOT EDIT this file directly. Any changes made to this file will be
#     overwritten during the next generation cycle.
#
# ----------------------------------------------------------------------------
subcategory: "Data Loss Prevention"
description: |-
  Allows creation of templates to de-identify content.
---</rdfs:comment>
  </owl:Class>
  <owl:DatatypeProperty rdf:about="http://example.org/onto/prop/google_data_loss_prevention_deidentify_template_create_time">
    <rdfs:label>create_time</rdfs:label>
    <rdfs:comment>The creation timestamp of an deidentifyTemplate. Set by the server.</rdfs:comment>
    <rdfs:domain rdf:resource="http://example.org/onto/class/google_data_loss_prevention_deidentify_template"/>
    <rdfs:range rdf:resource="http://www.w3.org/2001/XMLSchema#string"/>
  </owl:DatatypeProperty>
  <owl:DatatypeProperty rdf:about="http://example.org/onto/prop/google_data_loss_prevention_deidentify_template_description">
    <rdfs:label>description</rdfs:label>
    <rdfs:comment>A description of the template.</rdfs:comment>
    <rdfs:domain rdf:resource="http://example.org/onto/class/google_data_loss_prevention_deidentify_template"/>
    <rdfs:range rdf:resource="http://www.w3.org/2001/XMLSchema#string"/>
  </owl:DatatypeProperty>
  <owl:DatatypeProperty rdf:about="http://example.org/onto/prop/google_data_loss_prevention_deidentify_template_display_name">
    <rdfs:label>display_name</rdfs:label>
    <rdfs:comment>User set display name of the template.</rdfs:comment>
    <rdfs:domain rdf:resource="http://example.org/onto/class/google_data_loss_prevention_deidentify_template"/>
    <rdfs:range rdf:resource="http://www.w3.org/2001/XMLSchema#string"/>
  </owl:DatatypeProperty>
  <owl:DatatypeProperty rdf:about="http://example.org/onto/prop/google_data_loss_prevention_deidentify_template_id">
    <rdfs:label>id</rdfs:label>
    <rdfs:domain rdf:resource="http://example.org/onto/class/google_data_loss_prevention_deidentify_template"/>
    <rdfs:range rdf:resource="http://www.w3.org/2001/XMLSchema#string"/>
  </owl:DatatypeProperty>
  <owl:DatatypeProperty rdf:about="http://example.org/onto/prop/google_data_loss_prevention_deidentify_template_name">
    <rdfs:label>name</rdfs:label>
    <rdfs:comment>The resource name of the template. Set by the server.</rdfs:comment>
    <rdfs:domain rdf:resource="http://example.org/onto/class/google_data_loss_prevention_deidentify_template"/>
    <rdfs:range rdf:resource="http://www.w3.org/2001/XMLSchema#string"/>
  </owl:DatatypeProperty>
  <owl:DatatypeProperty rdf:about="http://example.org/onto/prop/google_data_loss_prevention_deidentify_template_parent">
    <rdfs:label>parent</rdfs:label>
    <rdfs:comment>The parent of the template in any of the following formats:

* 'projects/{{project}}'
* 'projects/{{project}}/locations/{{location}}'
* 'organizations/{{organization_id}}'
* 'organizations/{{organization_id}}/locations/{{location}}'</rdfs:comment>
    <rdfs:domain rdf:resource="http://example.org/onto/class/google_data_loss_prevention_deidentify_template"/>
    <rdfs:range rdf:resource="http://www.w3.org/2001/XMLSchema#string"/>
  </owl:DatatypeProperty>
  <owl:DatatypeProperty rdf:about="http://example.org/onto/prop/google_data_loss_prevention_deidentify_template_template_id">
    <rdfs:label>template_id</rdfs:label>
    <rdfs:comment>The template id can contain uppercase and lowercase letters, numbers, and hyphens;
that is, it must match the regular expression: [a-zA-Z\d-_]+. The maximum length is
100 characters. Can be empty to allow the system to generate one.</rdfs:comment>
    <rdfs:domain rdf:resource="http://example.org/onto/class/google_data_loss_prevention_deidentify_template"/>
    <rdfs:range rdf:resource="http://www.w3.org/2001/XMLSchema#string"/>
  </owl:DatatypeProperty>
  <owl:DatatypeProperty rdf:about="http://example.org/onto/prop/google_data_loss_prevention_deidentify_template_update_time">
    <rdfs:label>update_time</rdfs:label>
    <rdfs:comment>The last update timestamp of an deidentifyTemplate. Set by the server.</rdfs:comment>
    <rdfs:domain rdf:resource="http://example.org/onto/class/google_data_loss_prevention_deidentify_template"/>
    <rdfs:range rdf:resource="http://www.w3.org/2001/XMLSchema#string"/>
  </owl:DatatypeProperty>
  <owl:DatatypeProperty rdf:about="http://example.org/onto/prop/google_data_loss_prevention_deidentify_template_blue">
    <rdfs:label>blue</rdfs:label>
    <rdfs:comment>The amount of blue in the color as a value in the interval [0, 1].</rdfs:comment>
    <rdfs:domain rdf:resource="http://example.org/onto/class/google_data_loss_prevention_deidentify_template"/>
    <rdfs:range rdf:resource="http://www.w3.org/2001/XMLSchema#string"/>
  </owl:DatatypeProperty>
  <owl:DatatypeProperty rdf:about="http://example.org/onto/prop/google_data_loss_prevention_deidentify_template_green">
    <rdfs:label>green</rdfs:label>
    <rdfs:comment>The amount of green in the color as a value in the interval [0, 1].</rdfs:comment>
    <rdfs:domain rdf:resource="http://example.org/onto/class/google_data_loss_prevention_deidentify_template"/>
    <rdfs:range rdf:resource="http://www.w3.org/2001/XMLSchema#string"/>
  </owl:DatatypeProperty>
  <owl:DatatypeProperty rdf:about="http://example.org/onto/prop/google_data_loss_prevention_deidentify_template_red">
    <rdfs:label>red</rdfs:label>
    <rdfs:comment>The amount of red in the color as a value in the interval [0, 1].</rdfs:comment>
    <rdfs:domain rdf:resource="http://example.org/onto/class/google_data_loss_prevention_deidentify_template"/>
    <rdfs:range rdf:resource="http://www.w3.org/2001/XMLSchema#string"/>
  </owl:DatatypeProperty>
  <owl:DatatypeProperty rdf:about="http://example.org/onto/prop/google_data_loss_prevention_deidentify_template_name">
    <rdfs:label>name</rdfs:label>
    <rdfs:comment>Name of the information type.</rdfs:comment>
    <rdfs:domain rdf:resource="http://example.org/onto/class/google_data_loss_prevention_deidentify_template"/>
    <rdfs:range rdf:resource="http://www.w3.org/2001/XMLSchema#string"/>
  </owl:DatatypeProperty>
  <owl:DatatypeProperty rdf:about="http://example.org/onto/prop/google_data_loss_prevention_deidentify_template_version">
    <rdfs:label>version</rdfs:label>
    <rdfs:comment>Version name for this InfoType.</rdfs:comment>
    <rdfs:domain rdf:resource="http://example.org/onto/class/google_data_loss_prevention_deidentify_template"/>
    <rdfs:range rdf:resource="http://www.w3.org/2001/XMLSchema#string"/>
  </owl:DatatypeProperty>
  <owl:DatatypeProperty rdf:about="http://example.org/onto/prop/google_data_loss_prevention_deidentify_template_score">
    <rdfs:label>score</rdfs:label>
    <rdfs:comment>The sensitivity score applied to the resource. Possible values: ["SENSITIVITY_LOW", "SENSITIVITY_MODERATE", "SENSITIVITY_HIGH"]</rdfs:comment>
    <rdfs:domain rdf:resource="http://example.org/onto/class/google_data_loss_prevention_deidentify_template"/>
    <rdfs:range rdf:resource="http://www.w3.org/2001/XMLSchema#string"/>
  </owl:DatatypeProperty>
  <owl:DatatypeProperty rdf:about="http://example.org/onto/prop/google_data_loss_prevention_deidentify_template_name">
    <rdfs:label>name</rdfs:label>
    <rdfs:comment>Name of the information type.</rdfs:comment>
    <rdfs:domain rdf:resource="http://example.org/onto/class/google_data_loss_prevention_deidentify_template"/>
    <rdfs:range rdf:resource="http://www.w3.org/2001/XMLSchema#string"/>
  </owl:DatatypeProperty>
  <owl:DatatypeProperty rdf:about="http://example.org/onto/prop/google_data_loss_prevention_deidentify_template_version">
    <rdfs:label>version</rdfs:label>
    <rdfs:comment>Version name for this InfoType.</rdfs:comment>
    <rdfs:domain rdf:resource="http://example.org/onto/class/google_data_loss_prevention_deidentify_template"/>
    <rdfs:range rdf:resource="http://www.w3.org/2001/XMLSchema#string"/>
  </owl:DatatypeProperty>
  <owl:DatatypeProperty rdf:about="http://example.org/onto/prop/google_data_loss_prevention_deidentify_template_score">
    <rdfs:label>score</rdfs:label>
    <rdfs:comment>The sensitivity score applied to the resource. Possible values: ["SENSITIVITY_LOW", "SENSITIVITY_MODERATE", "SENSITIVITY_HIGH"]</rdfs:comment>
    <rdfs:domain rdf:resource="http://example.org/onto/class/google_data_loss_prevention_deidentify_template"/>
    <rdfs:range rdf:resource="http://www.w3.org/2001/XMLSchema#string"/>
  </owl:DatatypeProperty>
  <owl:DatatypeProperty rdf:about="http://example.org/onto/prop/google_data_loss_prevention_deidentify_template_replace_with_info_type_config">
    <rdfs:label>replace_with_info_type_config</rdfs:label>
    <rdfs:comment>Replace each matching finding with the name of the info type.</rdfs:comment>
    <rdfs:domain rdf:resource="http://example.org/onto/class/google_data_loss_prevention_deidentify_template"/>
    <rdfs:range rdf:resource="http://www.w3.org/2001/XMLSchema#string"/>
  </owl:DatatypeProperty>
  <owl:DatatypeProperty rdf:about="http://example.org/onto/prop/google_data_loss_prevention_deidentify_template_day_of_week_value">
    <rdfs:label>day_of_week_value</rdfs:label>
    <rdfs:comment>Represents a day of the week. Possible values: ["MONDAY", "TUESDAY", "WEDNESDAY", "THURSDAY", "FRIDAY", "SATURDAY", "SUNDAY"]</rdfs:comment>
    <rdfs:domain rdf:resource="http://example.org/onto/class/google_data_loss_prevention_deidentify_template"/>
    <rdfs:range rdf:resource="http://www.w3.org/2001/XMLSchema#string"/>
  </owl:DatatypeProperty>
  <owl:DatatypeProperty rdf:about="http://example.org/onto/prop/google_data_loss_prevention_deidentify_template_float_value">
    <rdfs:label>float_value</rdfs:label>
    <rdfs:comment>A float value.</rdfs:comment>
    <rdfs:domain rdf:resource="http://example.org/onto/class/google_data_loss_prevention_deidentify_template"/>
    <rdfs:range rdf:resource="http://www.w3.org/2001/XMLSchema#string"/>
  </owl:DatatypeProperty>
  <owl:DatatypeProperty rdf:about="http://example.org/onto/prop/google_data_loss_prevention_deidentify_template_integer_value">
    <rdfs:label>integer_value</rdfs:label>
    <rdfs:comment>An integer value (int64 format)</rdfs:comment>
    <rdfs:domain rdf:resource="http://example.org/onto/class/google_data_loss_prevention_deidentify_template"/>
    <rdfs:range rdf:resource="http://www.w3.org/2001/XMLSchema#string"/>
  </owl:DatatypeProperty>
  <owl:DatatypeProperty rdf:about="http://example.org/onto/prop/google_data_loss_prevention_deidentify_template_string_value">
    <rdfs:label>string_value</rdfs:label>
    <rdfs:comment>A string value.</rdfs:comment>
    <rdfs:domain rdf:resource="http://example.org/onto/class/google_data_loss_prevention_deidentify_template"/>
    <rdfs:range rdf:resource="http://www.w3.org/2001/XMLSchema#string"/>
  </owl:DatatypeProperty>
  <owl:DatatypeProperty rdf:about="http://example.org/onto/prop/google_data_loss_prevention_deidentify_template_timestamp_value">
    <rdfs:label>timestamp_value</rdfs:label>
    <rdfs:comment>A timestamp in RFC3339 UTC "Zulu" format, with nanosecond resolution and up to nine fractional digits. Examples: "2014-10-02T15:01:23Z" and "2014-10-02T15:01:23.045123456Z".</rdfs:comment>
    <rdfs:domain rdf:resource="http://example.org/onto/class/google_data_loss_prevention_deidentify_template"/>
    <rdfs:range rdf:resource="http://www.w3.org/2001/XMLSchema#string"/>
  </owl:DatatypeProperty>
  <owl:DatatypeProperty rdf:about="http://example.org/onto/prop/google_data_loss_prevention_deidentify_template_day">
    <rdfs:label>day</rdfs:label>
    <rdfs:comment>Day of a month. Must be from 1 to 31 and valid for the year and month, or 0 to specify a year by itself or a year and month where the day isn't significant.</rdfs:comment>
    <rdfs:domain rdf:resource="http://example.org/onto/class/google_data_loss_prevention_deidentify_template"/>
    <rdfs:range rdf:resource="http://www.w3.org/2001/XMLSchema#string"/>
  </owl:DatatypeProperty>
  <owl:DatatypeProperty rdf:about="http://example.org/onto/prop/google_data_loss_prevention_deidentify_template_month">
    <rdfs:label>month</rdfs:label>
    <rdfs:comment>Month of a year. Must be from 1 to 12, or 0 to specify a year without a month and day.</rdfs:comment>
    <rdfs:domain rdf:resource="http://example.org/onto/class/google_data_loss_prevention_deidentify_template"/>
    <rdfs:range rdf:resource="http://www.w3.org/2001/XMLSchema#string"/>
  </owl:DatatypeProperty>
  <owl:DatatypeProperty rdf:about="http://example.org/onto/prop/google_data_loss_prevention_deidentify_template_year">
    <rdfs:label>year</rdfs:label>
    <rdfs:comment>Year of the date. Must be from 1 to 9999, or 0 to specify a date without a year.</rdfs:comment>
    <rdfs:domain rdf:resource="http://example.org/onto/class/google_data_loss_prevention_deidentify_template"/>
    <rdfs:range rdf:resource="http://www.w3.org/2001/XMLSchema#string"/>
  </owl:DatatypeProperty>
  <owl:DatatypeProperty rdf:about="http://example.org/onto/prop/google_data_loss_prevention_deidentify_template_hours">
    <rdfs:label>hours</rdfs:label>
    <rdfs:comment>Hours of day in 24 hour format. Should be from 0 to 23. An API may choose to allow the value "24:00:00" for scenarios like business closing time.</rdfs:comment>
    <rdfs:domain rdf:resource="http://example.org/onto/class/google_data_loss_prevention_deidentify_template"/>
    <rdfs:range rdf:resource="http://www.w3.org/2001/XMLSchema#string"/>
  </owl:DatatypeProperty>
  <owl:DatatypeProperty rdf:about="http://example.org/onto/prop/google_data_loss_prevention_deidentify_template_minutes">
    <rdfs:label>minutes</rdfs:label>
    <rdfs:comment>Minutes of hour of day. Must be from 0 to 59.</rdfs:comment>
    <rdfs:domain rdf:resource="http://example.org/onto/class/google_data_loss_prevention_deidentify_template"/>
    <rdfs:range rdf:resource="http://www.w3.org/2001/XMLSchema#string"/>
  </owl:DatatypeProperty>
  <owl:DatatypeProperty rdf:about="http://example.org/onto/prop/google_data_loss_prevention_deidentify_template_nanos">
    <rdfs:label>nanos</rdfs:label>
    <rdfs:comment>Fractions of seconds in nanoseconds. Must be from 0 to 999,999,999.</rdfs:comment>
    <rdfs:domain rdf:resource="http://example.org/onto/class/google_data_loss_prevention_deidentify_template"/>
    <rdfs:range rdf:resource="http://www.w3.org/2001/XMLSchema#string"/>
  </owl:DatatypeProperty>
  <owl:DatatypeProperty rdf:about="http://example.org/onto/prop/google_data_loss_prevention_deidentify_template_seconds">
    <rdfs:label>seconds</rdfs:label>
    <rdfs:comment>Seconds of minutes of the time. Must normally be from 0 to 59. An API may allow the value 60 if it allows leap-seconds.</rdfs:comment>
    <rdfs:domain rdf:resource="http://example.org/onto/class/google_data_loss_prevention_deidentify_template"/>
    <rdfs:range rdf:resource="http://www.w3.org/2001/XMLSchema#string"/>
  </owl:DatatypeProperty>
  <owl:DatatypeProperty rdf:about="http://example.org/onto/prop/google_data_loss_prevention_deidentify_template_day_of_week_value">
    <rdfs:label>day_of_week_value</rdfs:label>
    <rdfs:comment>Represents a day of the week. Possible values: ["MONDAY", "TUESDAY", "WEDNESDAY", "THURSDAY", "FRIDAY", "SATURDAY", "SUNDAY"]</rdfs:comment>
    <rdfs:domain rdf:resource="http://example.org/onto/class/google_data_loss_prevention_deidentify_template"/>
    <rdfs:range rdf:resource="http://www.w3.org/2001/XMLSchema#string"/>
  </owl:DatatypeProperty>
  <owl:DatatypeProperty rdf:about="http://example.org/onto/prop/google_data_loss_prevention_deidentify_template_float_value">
    <rdfs:label>float_value</rdfs:label>
    <rdfs:comment>A float value.</rdfs:comment>
    <rdfs:domain rdf:resource="http://example.org/onto/class/google_data_loss_prevention_deidentify_template"/>
    <rdfs:range rdf:resource="http://www.w3.org/2001/XMLSchema#string"/>
  </owl:DatatypeProperty>
  <owl:DatatypeProperty rdf:about="http://example.org/onto/prop/google_data_loss_prevention_deidentify_template_integer_value">
    <rdfs:label>integer_value</rdfs:label>
    <rdfs:comment>An integer value (int64 format)</rdfs:comment>
    <rdfs:domain rdf:resource="http://example.org/onto/class/google_data_loss_prevention_deidentify_template"/>
    <rdfs:range rdf:resource="http://www.w3.org/2001/XMLSchema#string"/>
  </owl:DatatypeProperty>
  <owl:DatatypeProperty rdf:about="http://example.org/onto/prop/google_data_loss_prevention_deidentify_template_string_value">
    <rdfs:label>string_value</rdfs:label>
    <rdfs:comment>A string value.</rdfs:comment>
    <rdfs:domain rdf:resource="http://example.org/onto/class/google_data_loss_prevention_deidentify_template"/>
    <rdfs:range rdf:resource="http://www.w3.org/2001/XMLSchema#string"/>
  </owl:DatatypeProperty>
  <owl:DatatypeProperty rdf:about="http://example.org/onto/prop/google_data_loss_prevention_deidentify_template_timestamp_value">
    <rdfs:label>timestamp_value</rdfs:label>
    <rdfs:comment>A timestamp in RFC3339 UTC "Zulu" format, with nanosecond resolution and up to nine fractional digits. Examples: "2014-10-02T15:01:23Z" and "2014-10-02T15:01:23.045123456Z".</rdfs:comment>
    <rdfs:domain rdf:resource="http://example.org/onto/class/google_data_loss_prevention_deidentify_template"/>
    <rdfs:range rdf:resource="http://www.w3.org/2001/XMLSchema#string"/>
  </owl:DatatypeProperty>
  <owl:DatatypeProperty rdf:about="http://example.org/onto/prop/google_data_loss_prevention_deidentify_template_day">
    <rdfs:label>day</rdfs:label>
    <rdfs:comment>Day of a month. Must be from 1 to 31 and valid for the year and month, or 0 to specify a year by itself or a year and month where the day isn't significant.</rdfs:comment>
    <rdfs:domain rdf:resource="http://example.org/onto/class/google_data_loss_prevention_deidentify_template"/>
    <rdfs:range rdf:resource="http://www.w3.org/2001/XMLSchema#string"/>
  </owl:DatatypeProperty>
  <owl:DatatypeProperty rdf:about="http://example.org/onto/prop/google_data_loss_prevention_deidentify_template_month">
    <rdfs:label>month</rdfs:label>
    <rdfs:comment>Month of a year. Must be from 1 to 12, or 0 to specify a year without a month and day.</rdfs:comment>
    <rdfs:domain rdf:resource="http://example.org/onto/class/google_data_loss_prevention_deidentify_template"/>
    <rdfs:range rdf:resource="http://www.w3.org/2001/XMLSchema#string"/>
  </owl:DatatypeProperty>
  <owl:DatatypeProperty rdf:about="http://example.org/onto/prop/google_data_loss_prevention_deidentify_template_year">
    <rdfs:label>year</rdfs:label>
    <rdfs:comment>Year of the date. Must be from 1 to 9999, or 0 to specify a date without a year.</rdfs:comment>
    <rdfs:domain rdf:resource="http://example.org/onto/class/google_data_loss_prevention_deidentify_template"/>
    <rdfs:range rdf:resource="http://www.w3.org/2001/XMLSchema#string"/>
  </owl:DatatypeProperty>
  <owl:DatatypeProperty rdf:about="http://example.org/onto/prop/google_data_loss_prevention_deidentify_template_hours">
    <rdfs:label>hours</rdfs:label>
    <rdfs:comment>Hours of day in 24 hour format. Should be from 0 to 23. An API may choose to allow the value "24:00:00" for scenarios like business closing time.</rdfs:comment>
    <rdfs:domain rdf:resource="http://example.org/onto/class/google_data_loss_prevention_deidentify_template"/>
    <rdfs:range rdf:resource="http://www.w3.org/2001/XMLSchema#string"/>
  </owl:DatatypeProperty>
  <owl:DatatypeProperty rdf:about="http://example.org/onto/prop/google_data_loss_prevention_deidentify_template_minutes">
    <rdfs:label>minutes</rdfs:label>
    <rdfs:comment>Minutes of hour of day. Must be from 0 to 59.</rdfs:comment>
    <rdfs:domain rdf:resource="http://example.org/onto/class/google_data_loss_prevention_deidentify_template"/>
    <rdfs:range rdf:resource="http://www.w3.org/2001/XMLSchema#string"/>
  </owl:DatatypeProperty>
  <owl:DatatypeProperty rdf:about="http://example.org/onto/prop/google_data_loss_prevention_deidentify_template_nanos">
    <rdfs:label>nanos</rdfs:label>
    <rdfs:comment>Fractions of seconds in nanoseconds. Must be from 0 to 999,999,999.</rdfs:comment>
    <rdfs:domain rdf:resource="http://example.org/onto/class/google_data_loss_prevention_deidentify_template"/>
    <rdfs:range rdf:resource="http://www.w3.org/2001/XMLSchema#string"/>
  </owl:DatatypeProperty>
  <owl:DatatypeProperty rdf:about="http://example.org/onto/prop/google_data_loss_prevention_deidentify_template_seconds">
    <rdfs:label>seconds</rdfs:label>
    <rdfs:comment>Seconds of minutes of the time. Must normally be from 0 to 59. An API may allow the value 60 if it allows leap-seconds.</rdfs:comment>
    <rdfs:domain rdf:resource="http://example.org/onto/class/google_data_loss_prevention_deidentify_template"/>
    <rdfs:range rdf:resource="http://www.w3.org/2001/XMLSchema#string"/>
  </owl:DatatypeProperty>
  <owl:DatatypeProperty rdf:about="http://example.org/onto/prop/google_data_loss_prevention_deidentify_template_day_of_week_value">
    <rdfs:label>day_of_week_value</rdfs:label>
    <rdfs:comment>Represents a day of the week. Possible values: ["MONDAY", "TUESDAY", "WEDNESDAY", "THURSDAY", "FRIDAY", "SATURDAY", "SUNDAY"]</rdfs:comment>
    <rdfs:domain rdf:resource="http://example.org/onto/class/google_data_loss_prevention_deidentify_template"/>
    <rdfs:range rdf:resource="http://www.w3.org/2001/XMLSchema#string"/>
  </owl:DatatypeProperty>
  <owl:DatatypeProperty rdf:about="http://example.org/onto/prop/google_data_loss_prevention_deidentify_template_float_value">
    <rdfs:label>float_value</rdfs:label>
    <rdfs:comment>A float value.</rdfs:comment>
    <rdfs:domain rdf:resource="http://example.org/onto/class/google_data_loss_prevention_deidentify_template"/>
    <rdfs:range rdf:resource="http://www.w3.org/2001/XMLSchema#string"/>
  </owl:DatatypeProperty>
  <owl:DatatypeProperty rdf:about="http://example.org/onto/prop/google_data_loss_prevention_deidentify_template_integer_value">
    <rdfs:label>integer_value</rdfs:label>
    <rdfs:comment>An integer value (int64 format)</rdfs:comment>
    <rdfs:domain rdf:resource="http://example.org/onto/class/google_data_loss_prevention_deidentify_template"/>
    <rdfs:range rdf:resource="http://www.w3.org/2001/XMLSchema#string"/>
  </owl:DatatypeProperty>
  <owl:DatatypeProperty rdf:about="http://example.org/onto/prop/google_data_loss_prevention_deidentify_template_string_value">
    <rdfs:label>string_value</rdfs:label>
    <rdfs:comment>A string value.</rdfs:comment>
    <rdfs:domain rdf:resource="http://example.org/onto/class/google_data_loss_prevention_deidentify_template"/>
    <rdfs:range rdf:resource="http://www.w3.org/2001/XMLSchema#string"/>
  </owl:DatatypeProperty>
  <owl:DatatypeProperty rdf:about="http://example.org/onto/prop/google_data_loss_prevention_deidentify_template_timestamp_value">
    <rdfs:label>timestamp_value</rdfs:label>
    <rdfs:comment>A timestamp in RFC3339 UTC "Zulu" format, with nanosecond resolution and up to nine fractional digits. Examples: "2014-10-02T15:01:23Z" and "2014-10-02T15:01:23.045123456Z".</rdfs:comment>
    <rdfs:domain rdf:resource="http://example.org/onto/class/google_data_loss_prevention_deidentify_template"/>
    <rdfs:range rdf:resource="http://www.w3.org/2001/XMLSchema#string"/>
  </owl:DatatypeProperty>
  <owl:DatatypeProperty rdf:about="http://example.org/onto/prop/google_data_loss_prevention_deidentify_template_day">
    <rdfs:label>day</rdfs:label>
    <rdfs:comment>Day of a month. Must be from 1 to 31 and valid for the year and month, or 0 to specify a year by itself or a year and month where the day isn't significant.</rdfs:comment>
    <rdfs:domain rdf:resource="http://example.org/onto/class/google_data_loss_prevention_deidentify_template"/>
    <rdfs:range rdf:resource="http://www.w3.org/2001/XMLSchema#string"/>
  </owl:DatatypeProperty>
  <owl:DatatypeProperty rdf:about="http://example.org/onto/prop/google_data_loss_prevention_deidentify_template_month">
    <rdfs:label>month</rdfs:label>
    <rdfs:comment>Month of a year. Must be from 1 to 12, or 0 to specify a year without a month and day.</rdfs:comment>
    <rdfs:domain rdf:resource="http://example.org/onto/class/google_data_loss_prevention_deidentify_template"/>
    <rdfs:range rdf:resource="http://www.w3.org/2001/XMLSchema#string"/>
  </owl:DatatypeProperty>
  <owl:DatatypeProperty rdf:about="http://example.org/onto/prop/google_data_loss_prevention_deidentify_template_year">
    <rdfs:label>year</rdfs:label>
    <rdfs:comment>Year of the date. Must be from 1 to 9999, or 0 to specify a date without a year.</rdfs:comment>
    <rdfs:domain rdf:resource="http://example.org/onto/class/google_data_loss_prevention_deidentify_template"/>
    <rdfs:range rdf:resource="http://www.w3.org/2001/XMLSchema#string"/>
  </owl:DatatypeProperty>
  <owl:DatatypeProperty rdf:about="http://example.org/onto/prop/google_data_loss_prevention_deidentify_template_hours">
    <rdfs:label>hours</rdfs:label>
    <rdfs:comment>Hours of day in 24 hour format. Should be from 0 to 23. An API may choose to allow the value "24:00:00" for scenarios like business closing time.</rdfs:comment>
    <rdfs:domain rdf:resource="http://example.org/onto/class/google_data_loss_prevention_deidentify_template"/>
    <rdfs:range rdf:resource="http://www.w3.org/2001/XMLSchema#string"/>
  </owl:DatatypeProperty>
  <owl:DatatypeProperty rdf:about="http://example.org/onto/prop/google_data_loss_prevention_deidentify_template_minutes">
    <rdfs:label>minutes</rdfs:label>
    <rdfs:comment>Minutes of hour of day. Must be from 0 to 59.</rdfs:comment>
    <rdfs:domain rdf:resource="http://example.org/onto/class/google_data_loss_prevention_deidentify_template"/>
    <rdfs:range rdf:resource="http://www.w3.org/2001/XMLSchema#string"/>
  </owl:DatatypeProperty>
  <owl:DatatypeProperty rdf:about="http://example.org/onto/prop/google_data_loss_prevention_deidentify_template_nanos">
    <rdfs:label>nanos</rdfs:label>
    <rdfs:comment>Fractions of seconds in nanoseconds. Must be from 0 to 999,999,999.</rdfs:comment>
    <rdfs:domain rdf:resource="http://example.org/onto/class/google_data_loss_prevention_deidentify_template"/>
    <rdfs:range rdf:resource="http://www.w3.org/2001/XMLSchema#string"/>
  </owl:DatatypeProperty>
  <owl:DatatypeProperty rdf:about="http://example.org/onto/prop/google_data_loss_prevention_deidentify_template_seconds">
    <rdfs:label>seconds</rdfs:label>
    <rdfs:comment>Seconds of minutes of the time. Must normally be from 0 to 59. An API may allow the value 60 if it allows leap-seconds.</rdfs:comment>
    <rdfs:domain rdf:resource="http://example.org/onto/class/google_data_loss_prevention_deidentify_template"/>
    <rdfs:range rdf:resource="http://www.w3.org/2001/XMLSchema#string"/>
  </owl:DatatypeProperty>
  <owl:DatatypeProperty rdf:about="http://example.org/onto/prop/google_data_loss_prevention_deidentify_template_masking_character">
    <rdfs:label>masking_character</rdfs:label>
    <rdfs:comment>Character to use to mask the sensitive values—for example, * for an alphabetic string such as a name, or 0 for a numeric string
such as ZIP code or credit card number. This string must have a length of 1. If not supplied, this value defaults to * for
strings, and 0 for digits.</rdfs:comment>
    <rdfs:domain rdf:resource="http://example.org/onto/class/google_data_loss_prevention_deidentify_template"/>
    <rdfs:range rdf:resource="http://www.w3.org/2001/XMLSchema#string"/>
  </owl:DatatypeProperty>
  <owl:DatatypeProperty rdf:about="http://example.org/onto/prop/google_data_loss_prevention_deidentify_template_number_to_mask">
    <rdfs:label>number_to_mask</rdfs:label>
    <rdfs:comment>Number of characters to mask. If not set, all matching chars will be masked. Skipped characters do not count towards this tally.</rdfs:comment>
    <rdfs:domain rdf:resource="http://example.org/onto/class/google_data_loss_prevention_deidentify_template"/>
    <rdfs:range rdf:resource="http://www.w3.org/2001/XMLSchema#string"/>
  </owl:DatatypeProperty>
  <owl:DatatypeProperty rdf:about="http://example.org/onto/prop/google_data_loss_prevention_deidentify_template_reverse_order">
    <rdfs:label>reverse_order</rdfs:label>
    <rdfs:comment>Mask characters in reverse order. For example, if masking_character is 0, number_to_mask is 14, and reverse_order is 'false', then the
input string '1234-5678-9012-3456' is masked as '00000000000000-3456'.</rdfs:comment>
    <rdfs:domain rdf:resource="http://example.org/onto/class/google_data_loss_prevention_deidentify_template"/>
    <rdfs:range rdf:resource="http://www.w3.org/2001/XMLSchema#string"/>
  </owl:DatatypeProperty>
  <owl:DatatypeProperty rdf:about="http://example.org/onto/prop/google_data_loss_prevention_deidentify_template_characters_to_skip">
    <rdfs:label>characters_to_skip</rdfs:label>
    <rdfs:comment>Characters to not transform when masking.</rdfs:comment>
    <rdfs:domain rdf:resource="http://example.org/onto/class/google_data_loss_prevention_deidentify_template"/>
    <rdfs:range rdf:resource="http://www.w3.org/2001/XMLSchema#string"/>
  </owl:DatatypeProperty>
  <owl:DatatypeProperty rdf:about="http://example.org/onto/prop/google_data_loss_prevention_deidentify_template_common_characters_to_ignore">
    <rdfs:label>common_characters_to_ignore</rdfs:label>
    <rdfs:comment>Common characters to not transform when masking. Useful to avoid removing punctuation. Possible values: ["NUMERIC", "ALPHA_UPPER_CASE", "ALPHA_LOWER_CASE", "PUNCTUATION", "WHITESPACE"]</rdfs:comment>
    <rdfs:domain rdf:resource="http://example.org/onto/class/google_data_loss_prevention_deidentify_template"/>
    <rdfs:range rdf:resource="http://www.w3.org/2001/XMLSchema#string"/>
  </owl:DatatypeProperty>
  <owl:DatatypeProperty rdf:about="http://example.org/onto/prop/google_data_loss_prevention_deidentify_template_name">
    <rdfs:label>name</rdfs:label>
    <rdfs:comment>Name describing the field.</rdfs:comment>
    <rdfs:domain rdf:resource="http://example.org/onto/class/google_data_loss_prevention_deidentify_template"/>
    <rdfs:range rdf:resource="http://www.w3.org/2001/XMLSchema#string"/>
  </owl:DatatypeProperty>
  <owl:DatatypeProperty rdf:about="http://example.org/onto/prop/google_data_loss_prevention_deidentify_template_crypto_key_name">
    <rdfs:label>crypto_key_name</rdfs:label>
    <rdfs:comment>The resource name of the KMS CryptoKey to use for unwrapping.</rdfs:comment>
    <rdfs:domain rdf:resource="http://example.org/onto/class/google_data_loss_prevention_deidentify_template"/>
    <rdfs:range rdf:resource="http://www.w3.org/2001/XMLSchema#string"/>
  </owl:DatatypeProperty>
  <owl:DatatypeProperty rdf:about="http://example.org/onto/prop/google_data_loss_prevention_deidentify_template_wrapped_key">
    <rdfs:label>wrapped_key</rdfs:label>
    <rdfs:comment>The wrapped data crypto key.

A base64-encoded string.</rdfs:comment>
    <rdfs:domain rdf:resource="http://example.org/onto/class/google_data_loss_prevention_deidentify_template"/>
    <rdfs:range rdf:resource="http://www.w3.org/2001/XMLSchema#string"/>
  </owl:DatatypeProperty>
  <owl:DatatypeProperty rdf:about="http://example.org/onto/prop/google_data_loss_prevention_deidentify_template_name">
    <rdfs:label>name</rdfs:label>
    <rdfs:comment>Name of the key. This is an arbitrary string used to differentiate different keys. A unique key is generated per name: two separate 'TransientCryptoKey' protos share the same generated key if their names are the same. When the data crypto key is generated, this name is not used in any way (repeating the api call will result in a different key being generated).</rdfs:comment>
    <rdfs:domain rdf:resource="http://example.org/onto/class/google_data_loss_prevention_deidentify_template"/>
    <rdfs:range rdf:resource="http://www.w3.org/2001/XMLSchema#string"/>
  </owl:DatatypeProperty>
  <owl:DatatypeProperty rdf:about="http://example.org/onto/prop/google_data_loss_prevention_deidentify_template_key">
    <rdfs:label>key</rdfs:label>
    <rdfs:comment>A 128/192/256 bit key.

A base64-encoded string.</rdfs:comment>
    <rdfs:domain rdf:resource="http://example.org/onto/class/google_data_loss_prevention_deidentify_template"/>
    <rdfs:range rdf:resource="http://www.w3.org/2001/XMLSchema#string"/>
  </owl:DatatypeProperty>
  <owl:DatatypeProperty rdf:about="http://example.org/onto/prop/google_data_loss_prevention_deidentify_template_name">
    <rdfs:label>name</rdfs:label>
    <rdfs:comment>Name of the information type. Either a name of your choosing when creating a CustomInfoType, or one of the names listed at [https://cloud.google.com/dlp/docs/infotypes-reference](https://cloud.google.com/dlp/docs/infotypes-reference) when specifying a built-in type. When sending Cloud DLP results to Data Catalog, infoType names should conform to the pattern '[A-Za-z0-9$-_]{1,64}'.</rdfs:comment>
    <rdfs:domain rdf:resource="http://example.org/onto/class/google_data_loss_prevention_deidentify_template"/>
    <rdfs:range rdf:resource="http://www.w3.org/2001/XMLSchema#string"/>
  </owl:DatatypeProperty>
  <owl:DatatypeProperty rdf:about="http://example.org/onto/prop/google_data_loss_prevention_deidentify_template_version">
    <rdfs:label>version</rdfs:label>
    <rdfs:comment>Optional version name for this InfoType.</rdfs:comment>
    <rdfs:domain rdf:resource="http://example.org/onto/class/google_data_loss_prevention_deidentify_template"/>
    <rdfs:range rdf:resource="http://www.w3.org/2001/XMLSchema#string"/>
  </owl:DatatypeProperty>
  <owl:DatatypeProperty rdf:about="http://example.org/onto/prop/google_data_loss_prevention_deidentify_template_score">
    <rdfs:label>score</rdfs:label>
    <rdfs:comment>The sensitivity score applied to the resource. Possible values: ["SENSITIVITY_LOW", "SENSITIVITY_MODERATE", "SENSITIVITY_HIGH"]</rdfs:comment>
    <rdfs:domain rdf:resource="http://example.org/onto/class/google_data_loss_prevention_deidentify_template"/>
    <rdfs:range rdf:resource="http://www.w3.org/2001/XMLSchema#string"/>
  </owl:DatatypeProperty>
  <owl:DatatypeProperty rdf:about="http://example.org/onto/prop/google_data_loss_prevention_deidentify_template_crypto_key_name">
    <rdfs:label>crypto_key_name</rdfs:label>
    <rdfs:comment>The resource name of the KMS CryptoKey to use for unwrapping.</rdfs:comment>
    <rdfs:domain rdf:resource="http://example.org/onto/class/google_data_loss_prevention_deidentify_template"/>
    <rdfs:range rdf:resource="http://www.w3.org/2001/XMLSchema#string"/>
  </owl:DatatypeProperty>
  <owl:DatatypeProperty rdf:about="http://example.org/onto/prop/google_data_loss_prevention_deidentify_template_wrapped_key">
    <rdfs:label>wrapped_key</rdfs:label>
    <rdfs:comment>The wrapped data crypto key.

A base64-encoded string.</rdfs:comment>
    <rdfs:domain rdf:resource="http://example.org/onto/class/google_data_loss_prevention_deidentify_template"/>
    <rdfs:range rdf:resource="http://www.w3.org/2001/XMLSchema#string"/>
  </owl:DatatypeProperty>
  <owl:DatatypeProperty rdf:about="http://example.org/onto/prop/google_data_loss_prevention_deidentify_template_name">
    <rdfs:label>name</rdfs:label>
    <rdfs:comment>Name of the key. This is an arbitrary string used to differentiate different keys. A unique key is generated per name: two separate 'TransientCryptoKey' protos share the same generated key if their names are the same. When the data crypto key is generated, this name is not used in any way (repeating the api call will result in a different key being generated).</rdfs:comment>
    <rdfs:domain rdf:resource="http://example.org/onto/class/google_data_loss_prevention_deidentify_template"/>
    <rdfs:range rdf:resource="http://www.w3.org/2001/XMLSchema#string"/>
  </owl:DatatypeProperty>
  <owl:DatatypeProperty rdf:about="http://example.org/onto/prop/google_data_loss_prevention_deidentify_template_key">
    <rdfs:label>key</rdfs:label>
    <rdfs:comment>A 128/192/256 bit key.

A base64-encoded string.</rdfs:comment>
    <rdfs:domain rdf:resource="http://example.org/onto/class/google_data_loss_prevention_deidentify_template"/>
    <rdfs:range rdf:resource="http://www.w3.org/2001/XMLSchema#string"/>
  </owl:DatatypeProperty>
  <owl:DatatypeProperty rdf:about="http://example.org/onto/prop/google_data_loss_prevention_deidentify_template_common_alphabet">
    <rdfs:label>common_alphabet</rdfs:label>
    <rdfs:comment>Common alphabets. Possible values: ["FFX_COMMON_NATIVE_ALPHABET_UNSPECIFIED", "NUMERIC", "HEXADECIMAL", "UPPER_CASE_ALPHA_NUMERIC", "ALPHA_NUMERIC"]</rdfs:comment>
    <rdfs:domain rdf:resource="http://example.org/onto/class/google_data_loss_prevention_deidentify_template"/>
    <rdfs:range rdf:resource="http://www.w3.org/2001/XMLSchema#string"/>
  </owl:DatatypeProperty>
  <owl:DatatypeProperty rdf:about="http://example.org/onto/prop/google_data_loss_prevention_deidentify_template_custom_alphabet">
    <rdfs:label>custom_alphabet</rdfs:label>
    <rdfs:comment>This is supported by mapping these to the alphanumeric characters that the FFX mode natively supports. This happens before/after encryption/decryption. Each character listed must appear only once. Number of characters must be in the range \[2, 95\]. This must be encoded as ASCII. The order of characters does not matter. The full list of allowed characters is:

''0123456789ABCDEFGHIJKLMNOPQRSTUVWXYZabcdefghijklmnopqrstuvwxyz ~'!@#$%^&*()_-+={[}]|:;"'<,>.?/''</rdfs:comment>
    <rdfs:domain rdf:resource="http://example.org/onto/class/google_data_loss_prevention_deidentify_template"/>
    <rdfs:range rdf:resource="http://www.w3.org/2001/XMLSchema#string"/>
  </owl:DatatypeProperty>
  <owl:DatatypeProperty rdf:about="http://example.org/onto/prop/google_data_loss_prevention_deidentify_template_radix">
    <rdfs:label>radix</rdfs:label>
    <rdfs:comment>The native way to select the alphabet. Must be in the range \[2, 95\].</rdfs:comment>
    <rdfs:domain rdf:resource="http://example.org/onto/class/google_data_loss_prevention_deidentify_template"/>
    <rdfs:range rdf:resource="http://www.w3.org/2001/XMLSchema#string"/>
  </owl:DatatypeProperty>
  <owl:DatatypeProperty rdf:about="http://example.org/onto/prop/google_data_loss_prevention_deidentify_template_name">
    <rdfs:label>name</rdfs:label>
    <rdfs:comment>Name describing the field.</rdfs:comment>
    <rdfs:domain rdf:resource="http://example.org/onto/class/google_data_loss_prevention_deidentify_template"/>
    <rdfs:range rdf:resource="http://www.w3.org/2001/XMLSchema#string"/>
  </owl:DatatypeProperty>
  <owl:DatatypeProperty rdf:about="http://example.org/onto/prop/google_data_loss_prevention_deidentify_template_crypto_key_name">
    <rdfs:label>crypto_key_name</rdfs:label>
    <rdfs:comment>The resource name of the KMS CryptoKey to use for unwrapping.</rdfs:comment>
    <rdfs:domain rdf:resource="http://example.org/onto/class/google_data_loss_prevention_deidentify_template"/>
    <rdfs:range rdf:resource="http://www.w3.org/2001/XMLSchema#string"/>
  </owl:DatatypeProperty>
  <owl:DatatypeProperty rdf:about="http://example.org/onto/prop/google_data_loss_prevention_deidentify_template_wrapped_key">
    <rdfs:label>wrapped_key</rdfs:label>
    <rdfs:comment>The wrapped data crypto key.

A base64-encoded string.</rdfs:comment>
    <rdfs:domain rdf:resource="http://example.org/onto/class/google_data_loss_prevention_deidentify_template"/>
    <rdfs:range rdf:resource="http://www.w3.org/2001/XMLSchema#string"/>
  </owl:DatatypeProperty>
  <owl:DatatypeProperty rdf:about="http://example.org/onto/prop/google_data_loss_prevention_deidentify_template_name">
    <rdfs:label>name</rdfs:label>
    <rdfs:comment>Name of the key. This is an arbitrary string used to differentiate different keys. A unique key is generated per name: two separate 'TransientCryptoKey' protos share the same generated key if their names are the same. When the data crypto key is generated, this name is not used in any way (repeating the api call will result in a different key being generated).</rdfs:comment>
    <rdfs:domain rdf:resource="http://example.org/onto/class/google_data_loss_prevention_deidentify_template"/>
    <rdfs:range rdf:resource="http://www.w3.org/2001/XMLSchema#string"/>
  </owl:DatatypeProperty>
  <owl:DatatypeProperty rdf:about="http://example.org/onto/prop/google_data_loss_prevention_deidentify_template_key">
    <rdfs:label>key</rdfs:label>
    <rdfs:comment>A 128/192/256 bit key.

A base64-encoded string.</rdfs:comment>
    <rdfs:domain rdf:resource="http://example.org/onto/class/google_data_loss_prevention_deidentify_template"/>
    <rdfs:range rdf:resource="http://www.w3.org/2001/XMLSchema#string"/>
  </owl:DatatypeProperty>
  <owl:DatatypeProperty rdf:about="http://example.org/onto/prop/google_data_loss_prevention_deidentify_template_name">
    <rdfs:label>name</rdfs:label>
    <rdfs:comment>Name of the information type. Either a name of your choosing when creating a CustomInfoType, or one of the names listed at [https://cloud.google.com/dlp/docs/infotypes-reference](https://cloud.google.com/dlp/docs/infotypes-reference) when specifying a built-in type. When sending Cloud DLP results to Data Catalog, infoType names should conform to the pattern '[A-Za-z0-9$-_]{1,64}'.</rdfs:comment>
    <rdfs:domain rdf:resource="http://example.org/onto/class/google_data_loss_prevention_deidentify_template"/>
    <rdfs:range rdf:resource="http://www.w3.org/2001/XMLSchema#string"/>
  </owl:DatatypeProperty>
  <owl:DatatypeProperty rdf:about="http://example.org/onto/prop/google_data_loss_prevention_deidentify_template_version">
    <rdfs:label>version</rdfs:label>
    <rdfs:comment>Optional version name for this InfoType.</rdfs:comment>
    <rdfs:domain rdf:resource="http://example.org/onto/class/google_data_loss_prevention_deidentify_template"/>
    <rdfs:range rdf:resource="http://www.w3.org/2001/XMLSchema#string"/>
  </owl:DatatypeProperty>
  <owl:DatatypeProperty rdf:about="http://example.org/onto/prop/google_data_loss_prevention_deidentify_template_score">
    <rdfs:label>score</rdfs:label>
    <rdfs:comment>The sensitivity score applied to the resource. Possible values: ["SENSITIVITY_LOW", "SENSITIVITY_MODERATE", "SENSITIVITY_HIGH"]</rdfs:comment>
    <rdfs:domain rdf:resource="http://example.org/onto/class/google_data_loss_prevention_deidentify_template"/>
    <rdfs:range rdf:resource="http://www.w3.org/2001/XMLSchema#string"/>
  </owl:DatatypeProperty>
  <owl:DatatypeProperty rdf:about="http://example.org/onto/prop/google_data_loss_prevention_deidentify_template_lower_bound_days">
    <rdfs:label>lower_bound_days</rdfs:label>
    <rdfs:comment>Range of shift in days. Negative means shift to earlier in time.</rdfs:comment>
    <rdfs:domain rdf:resource="http://example.org/onto/class/google_data_loss_prevention_deidentify_template"/>
    <rdfs:range rdf:resource="http://www.w3.org/2001/XMLSchema#string"/>
  </owl:DatatypeProperty>
  <owl:DatatypeProperty rdf:about="http://example.org/onto/prop/google_data_loss_prevention_deidentify_template_upper_bound_days">
    <rdfs:label>upper_bound_days</rdfs:label>
    <rdfs:comment>Range of shift in days. Actual shift will be selected at random within this range (inclusive ends).
Negative means shift to earlier in time. Must not be more than 365250 days (1000 years) each direction.</rdfs:comment>
    <rdfs:domain rdf:resource="http://example.org/onto/class/google_data_loss_prevention_deidentify_template"/>
    <rdfs:range rdf:resource="http://www.w3.org/2001/XMLSchema#string"/>
  </owl:DatatypeProperty>
  <owl:DatatypeProperty rdf:about="http://example.org/onto/prop/google_data_loss_prevention_deidentify_template_name">
    <rdfs:label>name</rdfs:label>
    <rdfs:comment>Name describing the field.</rdfs:comment>
    <rdfs:domain rdf:resource="http://example.org/onto/class/google_data_loss_prevention_deidentify_template"/>
    <rdfs:range rdf:resource="http://www.w3.org/2001/XMLSchema#string"/>
  </owl:DatatypeProperty>
  <owl:DatatypeProperty rdf:about="http://example.org/onto/prop/google_data_loss_prevention_deidentify_template_crypto_key_name">
    <rdfs:label>crypto_key_name</rdfs:label>
    <rdfs:comment>The resource name of the KMS CryptoKey to use for unwrapping.</rdfs:comment>
    <rdfs:domain rdf:resource="http://example.org/onto/class/google_data_loss_prevention_deidentify_template"/>
    <rdfs:range rdf:resource="http://www.w3.org/2001/XMLSchema#string"/>
  </owl:DatatypeProperty>
  <owl:DatatypeProperty rdf:about="http://example.org/onto/prop/google_data_loss_prevention_deidentify_template_wrapped_key">
    <rdfs:label>wrapped_key</rdfs:label>
    <rdfs:comment>The wrapped data crypto key.
A base64-encoded string.</rdfs:comment>
    <rdfs:domain rdf:resource="http://example.org/onto/class/google_data_loss_prevention_deidentify_template"/>
    <rdfs:range rdf:resource="http://www.w3.org/2001/XMLSchema#string"/>
  </owl:DatatypeProperty>
  <owl:DatatypeProperty rdf:about="http://example.org/onto/prop/google_data_loss_prevention_deidentify_template_name">
    <rdfs:label>name</rdfs:label>
    <rdfs:comment>Name of the key. This is an arbitrary string used to differentiate different keys. A unique key is generated per name: two separate 'TransientCryptoKey' protos share the same generated key if their names are the same. When the data crypto key is generated, this name is not used in any way (repeating the api call will result in a different key being generated).</rdfs:comment>
    <rdfs:domain rdf:resource="http://example.org/onto/class/google_data_loss_prevention_deidentify_template"/>
    <rdfs:range rdf:resource="http://www.w3.org/2001/XMLSchema#string"/>
  </owl:DatatypeProperty>
  <owl:DatatypeProperty rdf:about="http://example.org/onto/prop/google_data_loss_prevention_deidentify_template_key">
    <rdfs:label>key</rdfs:label>
    <rdfs:comment>A 128/192/256 bit key.
A base64-encoded string.</rdfs:comment>
    <rdfs:domain rdf:resource="http://example.org/onto/class/google_data_loss_prevention_deidentify_template"/>
    <rdfs:range rdf:resource="http://www.w3.org/2001/XMLSchema#string"/>
  </owl:DatatypeProperty>
  <owl:DatatypeProperty rdf:about="http://example.org/onto/prop/google_data_loss_prevention_deidentify_template_bucket_size">
    <rdfs:label>bucket_size</rdfs:label>
    <rdfs:comment>Size of each bucket (except for minimum and maximum buckets).
So if lower_bound = 10, upper_bound = 89, and bucketSize = 10, then the following buckets would be used: -10, 10-20, 20-30, 30-40, 40-50, 50-60, 60-70, 70-80, 80-89, 89+.
Precision up to 2 decimals works.</rdfs:comment>
    <rdfs:domain rdf:resource="http://example.org/onto/class/google_data_loss_prevention_deidentify_template"/>
    <rdfs:range rdf:resource="http://www.w3.org/2001/XMLSchema#string"/>
  </owl:DatatypeProperty>
  <owl:DatatypeProperty rdf:about="http://example.org/onto/prop/google_data_loss_prevention_deidentify_template_float_value">
    <rdfs:label>float_value</rdfs:label>
    <rdfs:comment>A float value.</rdfs:comment>
    <rdfs:domain rdf:resource="http://example.org/onto/class/google_data_loss_prevention_deidentify_template"/>
    <rdfs:range rdf:resource="http://www.w3.org/2001/XMLSchema#string"/>
  </owl:DatatypeProperty>
  <owl:DatatypeProperty rdf:about="http://example.org/onto/prop/google_data_loss_prevention_deidentify_template_integer_value">
    <rdfs:label>integer_value</rdfs:label>
    <rdfs:comment>An integer value (int64 format)</rdfs:comment>
    <rdfs:domain rdf:resource="http://example.org/onto/class/google_data_loss_prevention_deidentify_template"/>
    <rdfs:range rdf:resource="http://www.w3.org/2001/XMLSchema#string"/>
  </owl:DatatypeProperty>
  <owl:DatatypeProperty rdf:about="http://example.org/onto/prop/google_data_loss_prevention_deidentify_template_float_value">
    <rdfs:label>float_value</rdfs:label>
    <rdfs:comment>A float value.</rdfs:comment>
    <rdfs:domain rdf:resource="http://example.org/onto/class/google_data_loss_prevention_deidentify_template"/>
    <rdfs:range rdf:resource="http://www.w3.org/2001/XMLSchema#string"/>
  </owl:DatatypeProperty>
  <owl:DatatypeProperty rdf:about="http://example.org/onto/prop/google_data_loss_prevention_deidentify_template_integer_value">
    <rdfs:label>integer_value</rdfs:label>
    <rdfs:comment>An integer value (int64 format)</rdfs:comment>
    <rdfs:domain rdf:resource="http://example.org/onto/class/google_data_loss_prevention_deidentify_template"/>
    <rdfs:range rdf:resource="http://www.w3.org/2001/XMLSchema#string"/>
  </owl:DatatypeProperty>
  <owl:DatatypeProperty rdf:about="http://example.org/onto/prop/google_data_loss_prevention_deidentify_template_boolean_value">
    <rdfs:label>boolean_value</rdfs:label>
    <rdfs:comment>A boolean value.</rdfs:comment>
    <rdfs:domain rdf:resource="http://example.org/onto/class/google_data_loss_prevention_deidentify_template"/>
    <rdfs:range rdf:resource="http://www.w3.org/2001/XMLSchema#string"/>
  </owl:DatatypeProperty>
  <owl:DatatypeProperty rdf:about="http://example.org/onto/prop/google_data_loss_prevention_deidentify_template_day_of_week_value">
    <rdfs:label>day_of_week_value</rdfs:label>
    <rdfs:comment>Represents a day of the week. Possible values: ["MONDAY", "TUESDAY", "WEDNESDAY", "THURSDAY", "FRIDAY", "SATURDAY", "SUNDAY"]</rdfs:comment>
    <rdfs:domain rdf:resource="http://example.org/onto/class/google_data_loss_prevention_deidentify_template"/>
    <rdfs:range rdf:resource="http://www.w3.org/2001/XMLSchema#string"/>
  </owl:DatatypeProperty>
  <owl:DatatypeProperty rdf:about="http://example.org/onto/prop/google_data_loss_prevention_deidentify_template_float_value">
    <rdfs:label>float_value</rdfs:label>
    <rdfs:comment>A float value.</rdfs:comment>
    <rdfs:domain rdf:resource="http://example.org/onto/class/google_data_loss_prevention_deidentify_template"/>
    <rdfs:range rdf:resource="http://www.w3.org/2001/XMLSchema#string"/>
  </owl:DatatypeProperty>
  <owl:DatatypeProperty rdf:about="http://example.org/onto/prop/google_data_loss_prevention_deidentify_template_integer_value">
    <rdfs:label>integer_value</rdfs:label>
    <rdfs:comment>An integer value.</rdfs:comment>
    <rdfs:domain rdf:resource="http://example.org/onto/class/google_data_loss_prevention_deidentify_template"/>
    <rdfs:range rdf:resource="http://www.w3.org/2001/XMLSchema#string"/>
  </owl:DatatypeProperty>
  <owl:DatatypeProperty rdf:about="http://example.org/onto/prop/google_data_loss_prevention_deidentify_template_string_value">
    <rdfs:label>string_value</rdfs:label>
    <rdfs:comment>A string value.</rdfs:comment>
    <rdfs:domain rdf:resource="http://example.org/onto/class/google_data_loss_prevention_deidentify_template"/>
    <rdfs:range rdf:resource="http://www.w3.org/2001/XMLSchema#string"/>
  </owl:DatatypeProperty>
  <owl:DatatypeProperty rdf:about="http://example.org/onto/prop/google_data_loss_prevention_deidentify_template_timestamp_value">
    <rdfs:label>timestamp_value</rdfs:label>
    <rdfs:comment>A timestamp in RFC3339 UTC "Zulu" format, with nanosecond resolution and up to nine fractional digits.
Examples: "2014-10-02T15:01:23Z" and "2014-10-02T15:01:23.045123456Z".</rdfs:comment>
    <rdfs:domain rdf:resource="http://example.org/onto/class/google_data_loss_prevention_deidentify_template"/>
    <rdfs:range rdf:resource="http://www.w3.org/2001/XMLSchema#string"/>
  </owl:DatatypeProperty>
  <owl:DatatypeProperty rdf:about="http://example.org/onto/prop/google_data_loss_prevention_deidentify_template_day">
    <rdfs:label>day</rdfs:label>
    <rdfs:comment>Day of month. Must be from 1 to 31 and valid for the year and month, or 0 if specifying a
year by itself or a year and month where the day is not significant.</rdfs:comment>
    <rdfs:domain rdf:resource="http://example.org/onto/class/google_data_loss_prevention_deidentify_template"/>
    <rdfs:range rdf:resource="http://www.w3.org/2001/XMLSchema#string"/>
  </owl:DatatypeProperty>
  <owl:DatatypeProperty rdf:about="http://example.org/onto/prop/google_data_loss_prevention_deidentify_template_month">
    <rdfs:label>month</rdfs:label>
    <rdfs:comment>Month of year. Must be from 1 to 12, or 0 if specifying a year without a month and day.</rdfs:comment>
    <rdfs:domain rdf:resource="http://example.org/onto/class/google_data_loss_prevention_deidentify_template"/>
    <rdfs:range rdf:resource="http://www.w3.org/2001/XMLSchema#string"/>
  </owl:DatatypeProperty>
  <owl:DatatypeProperty rdf:about="http://example.org/onto/prop/google_data_loss_prevention_deidentify_template_year">
    <rdfs:label>year</rdfs:label>
    <rdfs:comment>Year of date. Must be from 1 to 9999, or 0 if specifying a date without a year.</rdfs:comment>
    <rdfs:domain rdf:resource="http://example.org/onto/class/google_data_loss_prevention_deidentify_template"/>
    <rdfs:range rdf:resource="http://www.w3.org/2001/XMLSchema#string"/>
  </owl:DatatypeProperty>
  <owl:DatatypeProperty rdf:about="http://example.org/onto/prop/google_data_loss_prevention_deidentify_template_hours">
    <rdfs:label>hours</rdfs:label>
    <rdfs:comment>Hours of day in 24 hour format. Should be from 0 to 23.</rdfs:comment>
    <rdfs:domain rdf:resource="http://example.org/onto/class/google_data_loss_prevention_deidentify_template"/>
    <rdfs:range rdf:resource="http://www.w3.org/2001/XMLSchema#string"/>
  </owl:DatatypeProperty>
  <owl:DatatypeProperty rdf:about="http://example.org/onto/prop/google_data_loss_prevention_deidentify_template_minutes">
    <rdfs:label>minutes</rdfs:label>
    <rdfs:comment>Minutes of hour of day. Must be from 0 to 59.</rdfs:comment>
    <rdfs:domain rdf:resource="http://example.org/onto/class/google_data_loss_prevention_deidentify_template"/>
    <rdfs:range rdf:resource="http://www.w3.org/2001/XMLSchema#string"/>
  </owl:DatatypeProperty>
  <owl:DatatypeProperty rdf:about="http://example.org/onto/prop/google_data_loss_prevention_deidentify_template_nanos">
    <rdfs:label>nanos</rdfs:label>
    <rdfs:comment>Fractions of seconds in nanoseconds. Must be from 0 to 999,999,999.</rdfs:comment>
    <rdfs:domain rdf:resource="http://example.org/onto/class/google_data_loss_prevention_deidentify_template"/>
    <rdfs:range rdf:resource="http://www.w3.org/2001/XMLSchema#string"/>
  </owl:DatatypeProperty>
  <owl:DatatypeProperty rdf:about="http://example.org/onto/prop/google_data_loss_prevention_deidentify_template_seconds">
    <rdfs:label>seconds</rdfs:label>
    <rdfs:comment>Seconds of minutes of the time. Must normally be from 0 to 59.</rdfs:comment>
    <rdfs:domain rdf:resource="http://example.org/onto/class/google_data_loss_prevention_deidentify_template"/>
    <rdfs:range rdf:resource="http://www.w3.org/2001/XMLSchema#string"/>
  </owl:DatatypeProperty>
  <owl:DatatypeProperty rdf:about="http://example.org/onto/prop/google_data_loss_prevention_deidentify_template_words">
    <rdfs:label>words</rdfs:label>
    <rdfs:comment>Words or phrases defining the dictionary. The dictionary must contain at least one phrase and every phrase must contain at least 2 characters that are letters or digits.</rdfs:comment>
    <rdfs:domain rdf:resource="http://example.org/onto/class/google_data_loss_prevention_deidentify_template"/>
    <rdfs:range rdf:resource="http://www.w3.org/2001/XMLSchema#string"/>
  </owl:DatatypeProperty>
  <owl:DatatypeProperty rdf:about="http://example.org/onto/prop/google_data_loss_prevention_deidentify_template_part_to_extract">
    <rdfs:label>part_to_extract</rdfs:label>
    <rdfs:comment>The part of the time to keep. Possible values: ["YEAR", "MONTH", "DAY_OF_MONTH", "DAY_OF_WEEK", "WEEK_OF_YEAR", "HOUR_OF_DAY"]</rdfs:comment>
    <rdfs:domain rdf:resource="http://example.org/onto/class/google_data_loss_prevention_deidentify_template"/>
    <rdfs:range rdf:resource="http://www.w3.org/2001/XMLSchema#string"/>
  </owl:DatatypeProperty>
  <owl:DatatypeProperty rdf:about="http://example.org/onto/prop/google_data_loss_prevention_deidentify_template_logical_operator">
    <rdfs:label>logical_operator</rdfs:label>
    <rdfs:comment>The operator to apply to the result of conditions. Default and currently only supported value is AND Default value: "AND" Possible values: ["AND"]</rdfs:comment>
    <rdfs:domain rdf:resource="http://example.org/onto/class/google_data_loss_prevention_deidentify_template"/>
    <rdfs:range rdf:resource="http://www.w3.org/2001/XMLSchema#string"/>
  </owl:DatatypeProperty>
  <owl:DatatypeProperty rdf:about="http://example.org/onto/prop/google_data_loss_prevention_deidentify_template_operator">
    <rdfs:label>operator</rdfs:label>
    <rdfs:comment>Operator used to compare the field or infoType to the value. Possible values: ["EQUAL_TO", "NOT_EQUAL_TO", "GREATER_THAN", "LESS_THAN", "GREATER_THAN_OR_EQUALS", "LESS_THAN_OR_EQUALS", "EXISTS"]</rdfs:comment>
    <rdfs:domain rdf:resource="http://example.org/onto/class/google_data_loss_prevention_deidentify_template"/>
    <rdfs:range rdf:resource="http://www.w3.org/2001/XMLSchema#string"/>
  </owl:DatatypeProperty>
  <owl:DatatypeProperty rdf:about="http://example.org/onto/prop/google_data_loss_prevention_deidentify_template_name">
    <rdfs:label>name</rdfs:label>
    <rdfs:comment>Name describing the field.</rdfs:comment>
    <rdfs:domain rdf:resource="http://example.org/onto/class/google_data_loss_prevention_deidentify_template"/>
    <rdfs:range rdf:resource="http://www.w3.org/2001/XMLSchema#string"/>
  </owl:DatatypeProperty>
  <owl:DatatypeProperty rdf:about="http://example.org/onto/prop/google_data_loss_prevention_deidentify_template_boolean_value">
    <rdfs:label>boolean_value</rdfs:label>
    <rdfs:comment>A boolean value.</rdfs:comment>
    <rdfs:domain rdf:resource="http://example.org/onto/class/google_data_loss_prevention_deidentify_template"/>
    <rdfs:range rdf:resource="http://www.w3.org/2001/XMLSchema#string"/>
  </owl:DatatypeProperty>
  <owl:DatatypeProperty rdf:about="http://example.org/onto/prop/google_data_loss_prevention_deidentify_template_day_of_week_value">
    <rdfs:label>day_of_week_value</rdfs:label>
    <rdfs:comment>Represents a day of the week. Possible values: ["MONDAY", "TUESDAY", "WEDNESDAY", "THURSDAY", "FRIDAY", "SATURDAY", "SUNDAY"]</rdfs:comment>
    <rdfs:domain rdf:resource="http://example.org/onto/class/google_data_loss_prevention_deidentify_template"/>
    <rdfs:range rdf:resource="http://www.w3.org/2001/XMLSchema#string"/>
  </owl:DatatypeProperty>
  <owl:DatatypeProperty rdf:about="http://example.org/onto/prop/google_data_loss_prevention_deidentify_template_float_value">
    <rdfs:label>float_value</rdfs:label>
    <rdfs:comment>A float value.</rdfs:comment>
    <rdfs:domain rdf:resource="http://example.org/onto/class/google_data_loss_prevention_deidentify_template"/>
    <rdfs:range rdf:resource="http://www.w3.org/2001/XMLSchema#string"/>
  </owl:DatatypeProperty>
  <owl:DatatypeProperty rdf:about="http://example.org/onto/prop/google_data_loss_prevention_deidentify_template_integer_value">
    <rdfs:label>integer_value</rdfs:label>
    <rdfs:comment>An integer value (int64 format)</rdfs:comment>
    <rdfs:domain rdf:resource="http://example.org/onto/class/google_data_loss_prevention_deidentify_template"/>
    <rdfs:range rdf:resource="http://www.w3.org/2001/XMLSchema#string"/>
  </owl:DatatypeProperty>
  <owl:DatatypeProperty rdf:about="http://example.org/onto/prop/google_data_loss_prevention_deidentify_template_string_value">
    <rdfs:label>string_value</rdfs:label>
    <rdfs:comment>A string value.</rdfs:comment>
    <rdfs:domain rdf:resource="http://example.org/onto/class/google_data_loss_prevention_deidentify_template"/>
    <rdfs:range rdf:resource="http://www.w3.org/2001/XMLSchema#string"/>
  </owl:DatatypeProperty>
  <owl:DatatypeProperty rdf:about="http://example.org/onto/prop/google_data_loss_prevention_deidentify_template_timestamp_value">
    <rdfs:label>timestamp_value</rdfs:label>
    <rdfs:comment>A timestamp in RFC3339 UTC "Zulu" format, with nanosecond resolution and up to nine fractional digits. Examples: "2014-10-02T15:01:23Z" and "2014-10-02T15:01:23.045123456Z".</rdfs:comment>
    <rdfs:domain rdf:resource="http://example.org/onto/class/google_data_loss_prevention_deidentify_template"/>
    <rdfs:range rdf:resource="http://www.w3.org/2001/XMLSchema#string"/>
  </owl:DatatypeProperty>
  <owl:DatatypeProperty rdf:about="http://example.org/onto/prop/google_data_loss_prevention_deidentify_template_day">
    <rdfs:label>day</rdfs:label>
    <rdfs:comment>Day of a month. Must be from 1 to 31 and valid for the year and month, or 0 to specify a year by itself or a year and month where the day isn't significant.</rdfs:comment>
    <rdfs:domain rdf:resource="http://example.org/onto/class/google_data_loss_prevention_deidentify_template"/>
    <rdfs:range rdf:resource="http://www.w3.org/2001/XMLSchema#string"/>
  </owl:DatatypeProperty>
  <owl:DatatypeProperty rdf:about="http://example.org/onto/prop/google_data_loss_prevention_deidentify_template_month">
    <rdfs:label>month</rdfs:label>
    <rdfs:comment>Month of a year. Must be from 1 to 12, or 0 to specify a year without a month and day.</rdfs:comment>
    <rdfs:domain rdf:resource="http://example.org/onto/class/google_data_loss_prevention_deidentify_template"/>
    <rdfs:range rdf:resource="http://www.w3.org/2001/XMLSchema#string"/>
  </owl:DatatypeProperty>
  <owl:DatatypeProperty rdf:about="http://example.org/onto/prop/google_data_loss_prevention_deidentify_template_year">
    <rdfs:label>year</rdfs:label>
    <rdfs:comment>Year of the date. Must be from 1 to 9999, or 0 to specify a date without a year.</rdfs:comment>
    <rdfs:domain rdf:resource="http://example.org/onto/class/google_data_loss_prevention_deidentify_template"/>
    <rdfs:range rdf:resource="http://www.w3.org/2001/XMLSchema#string"/>
  </owl:DatatypeProperty>
  <owl:DatatypeProperty rdf:about="http://example.org/onto/prop/google_data_loss_prevention_deidentify_template_hours">
    <rdfs:label>hours</rdfs:label>
    <rdfs:comment>Hours of day in 24 hour format. Should be from 0 to 23. An API may choose to allow the value "24:00:00" for scenarios like business closing time.</rdfs:comment>
    <rdfs:domain rdf:resource="http://example.org/onto/class/google_data_loss_prevention_deidentify_template"/>
    <rdfs:range rdf:resource="http://www.w3.org/2001/XMLSchema#string"/>
  </owl:DatatypeProperty>
  <owl:DatatypeProperty rdf:about="http://example.org/onto/prop/google_data_loss_prevention_deidentify_template_minutes">
    <rdfs:label>minutes</rdfs:label>
    <rdfs:comment>Minutes of hour of day. Must be from 0 to 59.</rdfs:comment>
    <rdfs:domain rdf:resource="http://example.org/onto/class/google_data_loss_prevention_deidentify_template"/>
    <rdfs:range rdf:resource="http://www.w3.org/2001/XMLSchema#string"/>
  </owl:DatatypeProperty>
  <owl:DatatypeProperty rdf:about="http://example.org/onto/prop/google_data_loss_prevention_deidentify_template_nanos">
    <rdfs:label>nanos</rdfs:label>
    <rdfs:comment>Fractions of seconds in nanoseconds. Must be from 0 to 999,999,999.</rdfs:comment>
    <rdfs:domain rdf:resource="http://example.org/onto/class/google_data_loss_prevention_deidentify_template"/>
    <rdfs:range rdf:resource="http://www.w3.org/2001/XMLSchema#string"/>
  </owl:DatatypeProperty>
  <owl:DatatypeProperty rdf:about="http://example.org/onto/prop/google_data_loss_prevention_deidentify_template_seconds">
    <rdfs:label>seconds</rdfs:label>
    <rdfs:comment>Seconds of minutes of the time. Must normally be from 0 to 59. An API may allow the value 60 if it allows leap-seconds.</rdfs:comment>
    <rdfs:domain rdf:resource="http://example.org/onto/class/google_data_loss_prevention_deidentify_template"/>
    <rdfs:range rdf:resource="http://www.w3.org/2001/XMLSchema#string"/>
  </owl:DatatypeProperty>
  <owl:DatatypeProperty rdf:about="http://example.org/onto/prop/google_data_loss_prevention_deidentify_template_name">
    <rdfs:label>name</rdfs:label>
    <rdfs:comment>Name describing the field.</rdfs:comment>
    <rdfs:domain rdf:resource="http://example.org/onto/class/google_data_loss_prevention_deidentify_template"/>
    <rdfs:range rdf:resource="http://www.w3.org/2001/XMLSchema#string"/>
  </owl:DatatypeProperty>
  <owl:DatatypeProperty rdf:about="http://example.org/onto/prop/google_data_loss_prevention_deidentify_template_name">
    <rdfs:label>name</rdfs:label>
    <rdfs:comment>Name of the information type.</rdfs:comment>
    <rdfs:domain rdf:resource="http://example.org/onto/class/google_data_loss_prevention_deidentify_template"/>
    <rdfs:range rdf:resource="http://www.w3.org/2001/XMLSchema#string"/>
  </owl:DatatypeProperty>
  <owl:DatatypeProperty rdf:about="http://example.org/onto/prop/google_data_loss_prevention_deidentify_template_version">
    <rdfs:label>version</rdfs:label>
    <rdfs:comment>Version name for this InfoType.</rdfs:comment>
    <rdfs:domain rdf:resource="http://example.org/onto/class/google_data_loss_prevention_deidentify_template"/>
    <rdfs:range rdf:resource="http://www.w3.org/2001/XMLSchema#string"/>
  </owl:DatatypeProperty>
  <owl:DatatypeProperty rdf:about="http://example.org/onto/prop/google_data_loss_prevention_deidentify_template_score">
    <rdfs:label>score</rdfs:label>
    <rdfs:comment>The sensitivity score applied to the resource. Possible values: ["SENSITIVITY_LOW", "SENSITIVITY_MODERATE", "SENSITIVITY_HIGH"]</rdfs:comment>
    <rdfs:domain rdf:resource="http://example.org/onto/class/google_data_loss_prevention_deidentify_template"/>
    <rdfs:range rdf:resource="http://www.w3.org/2001/XMLSchema#string"/>
  </owl:DatatypeProperty>
  <owl:DatatypeProperty rdf:about="http://example.org/onto/prop/google_data_loss_prevention_deidentify_template_day_of_week_value">
    <rdfs:label>day_of_week_value</rdfs:label>
    <rdfs:comment>Represents a day of the week. Possible values: ["MONDAY", "TUESDAY", "WEDNESDAY", "THURSDAY", "FRIDAY", "SATURDAY", "SUNDAY"]</rdfs:comment>
    <rdfs:domain rdf:resource="http://example.org/onto/class/google_data_loss_prevention_deidentify_template"/>
    <rdfs:range rdf:resource="http://www.w3.org/2001/XMLSchema#string"/>
  </owl:DatatypeProperty>
  <owl:DatatypeProperty rdf:about="http://example.org/onto/prop/google_data_loss_prevention_deidentify_template_float_value">
    <rdfs:label>float_value</rdfs:label>
    <rdfs:comment>A float value.</rdfs:comment>
    <rdfs:domain rdf:resource="http://example.org/onto/class/google_data_loss_prevention_deidentify_template"/>
    <rdfs:range rdf:resource="http://www.w3.org/2001/XMLSchema#string"/>
  </owl:DatatypeProperty>
  <owl:DatatypeProperty rdf:about="http://example.org/onto/prop/google_data_loss_prevention_deidentify_template_integer_value">
    <rdfs:label>integer_value</rdfs:label>
    <rdfs:comment>An integer value (int64 format)</rdfs:comment>
    <rdfs:domain rdf:resource="http://example.org/onto/class/google_data_loss_prevention_deidentify_template"/>
    <rdfs:range rdf:resource="http://www.w3.org/2001/XMLSchema#string"/>
  </owl:DatatypeProperty>
  <owl:DatatypeProperty rdf:about="http://example.org/onto/prop/google_data_loss_prevention_deidentify_template_string_value">
    <rdfs:label>string_value</rdfs:label>
    <rdfs:comment>A string value.</rdfs:comment>
    <rdfs:domain rdf:resource="http://example.org/onto/class/google_data_loss_prevention_deidentify_template"/>
    <rdfs:range rdf:resource="http://www.w3.org/2001/XMLSchema#string"/>
  </owl:DatatypeProperty>
  <owl:DatatypeProperty rdf:about="http://example.org/onto/prop/google_data_loss_prevention_deidentify_template_timestamp_value">
    <rdfs:label>timestamp_value</rdfs:label>
    <rdfs:comment>A timestamp in RFC3339 UTC "Zulu" format, with nanosecond resolution and up to nine fractional digits. Examples: "2014-10-02T15:01:23Z" and "2014-10-02T15:01:23.045123456Z".</rdfs:comment>
    <rdfs:domain rdf:resource="http://example.org/onto/class/google_data_loss_prevention_deidentify_template"/>
    <rdfs:range rdf:resource="http://www.w3.org/2001/XMLSchema#string"/>
  </owl:DatatypeProperty>
  <owl:DatatypeProperty rdf:about="http://example.org/onto/prop/google_data_loss_prevention_deidentify_template_day">
    <rdfs:label>day</rdfs:label>
    <rdfs:comment>Day of a month. Must be from 1 to 31 and valid for the year and month, or 0 to specify a year by itself or a year and month where the day isn't significant.</rdfs:comment>
    <rdfs:domain rdf:resource="http://example.org/onto/class/google_data_loss_prevention_deidentify_template"/>
    <rdfs:range rdf:resource="http://www.w3.org/2001/XMLSchema#string"/>
  </owl:DatatypeProperty>
  <owl:DatatypeProperty rdf:about="http://example.org/onto/prop/google_data_loss_prevention_deidentify_template_month">
    <rdfs:label>month</rdfs:label>
    <rdfs:comment>Month of a year. Must be from 1 to 12, or 0 to specify a year without a month and day.</rdfs:comment>
    <rdfs:domain rdf:resource="http://example.org/onto/class/google_data_loss_prevention_deidentify_template"/>
    <rdfs:range rdf:resource="http://www.w3.org/2001/XMLSchema#string"/>
  </owl:DatatypeProperty>
  <owl:DatatypeProperty rdf:about="http://example.org/onto/prop/google_data_loss_prevention_deidentify_template_year">
    <rdfs:label>year</rdfs:label>
    <rdfs:comment>Year of the date. Must be from 1 to 9999, or 0 to specify a date without a year.</rdfs:comment>
    <rdfs:domain rdf:resource="http://example.org/onto/class/google_data_loss_prevention_deidentify_template"/>
    <rdfs:range rdf:resource="http://www.w3.org/2001/XMLSchema#string"/>
  </owl:DatatypeProperty>
  <owl:DatatypeProperty rdf:about="http://example.org/onto/prop/google_data_loss_prevention_deidentify_template_hours">
    <rdfs:label>hours</rdfs:label>
    <rdfs:comment>Hours of day in 24 hour format. Should be from 0 to 23. An API may choose to allow the value "24:00:00" for scenarios like business closing time.</rdfs:comment>
    <rdfs:domain rdf:resource="http://example.org/onto/class/google_data_loss_prevention_deidentify_template"/>
    <rdfs:range rdf:resource="http://www.w3.org/2001/XMLSchema#string"/>
  </owl:DatatypeProperty>
  <owl:DatatypeProperty rdf:about="http://example.org/onto/prop/google_data_loss_prevention_deidentify_template_minutes">
    <rdfs:label>minutes</rdfs:label>
    <rdfs:comment>Minutes of hour of day. Must be from 0 to 59.</rdfs:comment>
    <rdfs:domain rdf:resource="http://example.org/onto/class/google_data_loss_prevention_deidentify_template"/>
    <rdfs:range rdf:resource="http://www.w3.org/2001/XMLSchema#string"/>
  </owl:DatatypeProperty>
  <owl:DatatypeProperty rdf:about="http://example.org/onto/prop/google_data_loss_prevention_deidentify_template_nanos">
    <rdfs:label>nanos</rdfs:label>
    <rdfs:comment>Fractions of seconds in nanoseconds. Must be from 0 to 999,999,999.</rdfs:comment>
    <rdfs:domain rdf:resource="http://example.org/onto/class/google_data_loss_prevention_deidentify_template"/>
    <rdfs:range rdf:resource="http://www.w3.org/2001/XMLSchema#string"/>
  </owl:DatatypeProperty>
  <owl:DatatypeProperty rdf:about="http://example.org/onto/prop/google_data_loss_prevention_deidentify_template_seconds">
    <rdfs:label>seconds</rdfs:label>
    <rdfs:comment>Seconds of minutes of the time. Must normally be from 0 to 59. An API may allow the value 60 if it allows leap-seconds.</rdfs:comment>
    <rdfs:domain rdf:resource="http://example.org/onto/class/google_data_loss_prevention_deidentify_template"/>
    <rdfs:range rdf:resource="http://www.w3.org/2001/XMLSchema#string"/>
  </owl:DatatypeProperty>
  <owl:DatatypeProperty rdf:about="http://example.org/onto/prop/google_data_loss_prevention_deidentify_template_day_of_week_value">
    <rdfs:label>day_of_week_value</rdfs:label>
    <rdfs:comment>Represents a day of the week. Possible values: ["MONDAY", "TUESDAY", "WEDNESDAY", "THURSDAY", "FRIDAY", "SATURDAY", "SUNDAY"]</rdfs:comment>
    <rdfs:domain rdf:resource="http://example.org/onto/class/google_data_loss_prevention_deidentify_template"/>
    <rdfs:range rdf:resource="http://www.w3.org/2001/XMLSchema#string"/>
  </owl:DatatypeProperty>
  <owl:DatatypeProperty rdf:about="http://example.org/onto/prop/google_data_loss_prevention_deidentify_template_float_value">
    <rdfs:label>float_value</rdfs:label>
    <rdfs:comment>A float value.</rdfs:comment>
    <rdfs:domain rdf:resource="http://example.org/onto/class/google_data_loss_prevention_deidentify_template"/>
    <rdfs:range rdf:resource="http://www.w3.org/2001/XMLSchema#string"/>
  </owl:DatatypeProperty>
  <owl:DatatypeProperty rdf:about="http://example.org/onto/prop/google_data_loss_prevention_deidentify_template_integer_value">
    <rdfs:label>integer_value</rdfs:label>
    <rdfs:comment>An integer value (int64 format)</rdfs:comment>
    <rdfs:domain rdf:resource="http://example.org/onto/class/google_data_loss_prevention_deidentify_template"/>
    <rdfs:range rdf:resource="http://www.w3.org/2001/XMLSchema#string"/>
  </owl:DatatypeProperty>
  <owl:DatatypeProperty rdf:about="http://example.org/onto/prop/google_data_loss_prevention_deidentify_template_string_value">
    <rdfs:label>string_value</rdfs:label>
    <rdfs:comment>A string value.</rdfs:comment>
    <rdfs:domain rdf:resource="http://example.org/onto/class/google_data_loss_prevention_deidentify_template"/>
    <rdfs:range rdf:resource="http://www.w3.org/2001/XMLSchema#string"/>
  </owl:DatatypeProperty>
  <owl:DatatypeProperty rdf:about="http://example.org/onto/prop/google_data_loss_prevention_deidentify_template_timestamp_value">
    <rdfs:label>timestamp_value</rdfs:label>
    <rdfs:comment>A timestamp in RFC3339 UTC "Zulu" format, with nanosecond resolution and up to nine fractional digits. Examples: "2014-10-02T15:01:23Z" and "2014-10-02T15:01:23.045123456Z".</rdfs:comment>
    <rdfs:domain rdf:resource="http://example.org/onto/class/google_data_loss_prevention_deidentify_template"/>
    <rdfs:range rdf:resource="http://www.w3.org/2001/XMLSchema#string"/>
  </owl:DatatypeProperty>
  <owl:DatatypeProperty rdf:about="http://example.org/onto/prop/google_data_loss_prevention_deidentify_template_day">
    <rdfs:label>day</rdfs:label>
    <rdfs:comment>Day of a month. Must be from 1 to 31 and valid for the year and month, or 0 to specify a year by itself or a year and month where the day isn't significant.</rdfs:comment>
    <rdfs:domain rdf:resource="http://example.org/onto/class/google_data_loss_prevention_deidentify_template"/>
    <rdfs:range rdf:resource="http://www.w3.org/2001/XMLSchema#string"/>
  </owl:DatatypeProperty>
  <owl:DatatypeProperty rdf:about="http://example.org/onto/prop/google_data_loss_prevention_deidentify_template_month">
    <rdfs:label>month</rdfs:label>
    <rdfs:comment>Month of a year. Must be from 1 to 12, or 0 to specify a year without a month and day.</rdfs:comment>
    <rdfs:domain rdf:resource="http://example.org/onto/class/google_data_loss_prevention_deidentify_template"/>
    <rdfs:range rdf:resource="http://www.w3.org/2001/XMLSchema#string"/>
  </owl:DatatypeProperty>
  <owl:DatatypeProperty rdf:about="http://example.org/onto/prop/google_data_loss_prevention_deidentify_template_year">
    <rdfs:label>year</rdfs:label>
    <rdfs:comment>Year of the date. Must be from 1 to 9999, or 0 to specify a date without a year.</rdfs:comment>
    <rdfs:domain rdf:resource="http://example.org/onto/class/google_data_loss_prevention_deidentify_template"/>
    <rdfs:range rdf:resource="http://www.w3.org/2001/XMLSchema#string"/>
  </owl:DatatypeProperty>
  <owl:DatatypeProperty rdf:about="http://example.org/onto/prop/google_data_loss_prevention_deidentify_template_hours">
    <rdfs:label>hours</rdfs:label>
    <rdfs:comment>Hours of day in 24 hour format. Should be from 0 to 23. An API may choose to allow the value "24:00:00" for scenarios like business closing time.</rdfs:comment>
    <rdfs:domain rdf:resource="http://example.org/onto/class/google_data_loss_prevention_deidentify_template"/>
    <rdfs:range rdf:resource="http://www.w3.org/2001/XMLSchema#string"/>
  </owl:DatatypeProperty>
  <owl:DatatypeProperty rdf:about="http://example.org/onto/prop/google_data_loss_prevention_deidentify_template_minutes">
    <rdfs:label>minutes</rdfs:label>
    <rdfs:comment>Minutes of hour of day. Must be from 0 to 59.</rdfs:comment>
    <rdfs:domain rdf:resource="http://example.org/onto/class/google_data_loss_prevention_deidentify_template"/>
    <rdfs:range rdf:resource="http://www.w3.org/2001/XMLSchema#string"/>
  </owl:DatatypeProperty>
  <owl:DatatypeProperty rdf:about="http://example.org/onto/prop/google_data_loss_prevention_deidentify_template_nanos">
    <rdfs:label>nanos</rdfs:label>
    <rdfs:comment>Fractions of seconds in nanoseconds. Must be from 0 to 999,999,999.</rdfs:comment>
    <rdfs:domain rdf:resource="http://example.org/onto/class/google_data_loss_prevention_deidentify_template"/>
    <rdfs:range rdf:resource="http://www.w3.org/2001/XMLSchema#string"/>
  </owl:DatatypeProperty>
  <owl:DatatypeProperty rdf:about="http://example.org/onto/prop/google_data_loss_prevention_deidentify_template_seconds">
    <rdfs:label>seconds</rdfs:label>
    <rdfs:comment>Seconds of minutes of the time. Must normally be from 0 to 59. An API may allow the value 60 if it allows leap-seconds.</rdfs:comment>
    <rdfs:domain rdf:resource="http://example.org/onto/class/google_data_loss_prevention_deidentify_template"/>
    <rdfs:range rdf:resource="http://www.w3.org/2001/XMLSchema#string"/>
  </owl:DatatypeProperty>
  <owl:DatatypeProperty rdf:about="http://example.org/onto/prop/google_data_loss_prevention_deidentify_template_day_of_week_value">
    <rdfs:label>day_of_week_value</rdfs:label>
    <rdfs:comment>Represents a day of the week. Possible values: ["MONDAY", "TUESDAY", "WEDNESDAY", "THURSDAY", "FRIDAY", "SATURDAY", "SUNDAY"]</rdfs:comment>
    <rdfs:domain rdf:resource="http://example.org/onto/class/google_data_loss_prevention_deidentify_template"/>
    <rdfs:range rdf:resource="http://www.w3.org/2001/XMLSchema#string"/>
  </owl:DatatypeProperty>
  <owl:DatatypeProperty rdf:about="http://example.org/onto/prop/google_data_loss_prevention_deidentify_template_float_value">
    <rdfs:label>float_value</rdfs:label>
    <rdfs:comment>A float value.</rdfs:comment>
    <rdfs:domain rdf:resource="http://example.org/onto/class/google_data_loss_prevention_deidentify_template"/>
    <rdfs:range rdf:resource="http://www.w3.org/2001/XMLSchema#string"/>
  </owl:DatatypeProperty>
  <owl:DatatypeProperty rdf:about="http://example.org/onto/prop/google_data_loss_prevention_deidentify_template_integer_value">
    <rdfs:label>integer_value</rdfs:label>
    <rdfs:comment>An integer value (int64 format)</rdfs:comment>
    <rdfs:domain rdf:resource="http://example.org/onto/class/google_data_loss_prevention_deidentify_template"/>
    <rdfs:range rdf:resource="http://www.w3.org/2001/XMLSchema#string"/>
  </owl:DatatypeProperty>
  <owl:DatatypeProperty rdf:about="http://example.org/onto/prop/google_data_loss_prevention_deidentify_template_string_value">
    <rdfs:label>string_value</rdfs:label>
    <rdfs:comment>A string value.</rdfs:comment>
    <rdfs:domain rdf:resource="http://example.org/onto/class/google_data_loss_prevention_deidentify_template"/>
    <rdfs:range rdf:resource="http://www.w3.org/2001/XMLSchema#string"/>
  </owl:DatatypeProperty>
  <owl:DatatypeProperty rdf:about="http://example.org/onto/prop/google_data_loss_prevention_deidentify_template_timestamp_value">
    <rdfs:label>timestamp_value</rdfs:label>
    <rdfs:comment>A timestamp in RFC3339 UTC "Zulu" format, with nanosecond resolution and up to nine fractional digits. Examples: "2014-10-02T15:01:23Z" and "2014-10-02T15:01:23.045123456Z".</rdfs:comment>
    <rdfs:domain rdf:resource="http://example.org/onto/class/google_data_loss_prevention_deidentify_template"/>
    <rdfs:range rdf:resource="http://www.w3.org/2001/XMLSchema#string"/>
  </owl:DatatypeProperty>
  <owl:DatatypeProperty rdf:about="http://example.org/onto/prop/google_data_loss_prevention_deidentify_template_day">
    <rdfs:label>day</rdfs:label>
    <rdfs:comment>Day of a month. Must be from 1 to 31 and valid for the year and month, or 0 to specify a year by itself or a year and month where the day isn't significant.</rdfs:comment>
    <rdfs:domain rdf:resource="http://example.org/onto/class/google_data_loss_prevention_deidentify_template"/>
    <rdfs:range rdf:resource="http://www.w3.org/2001/XMLSchema#string"/>
  </owl:DatatypeProperty>
  <owl:DatatypeProperty rdf:about="http://example.org/onto/prop/google_data_loss_prevention_deidentify_template_month">
    <rdfs:label>month</rdfs:label>
    <rdfs:comment>Month of a year. Must be from 1 to 12, or 0 to specify a year without a month and day.</rdfs:comment>
    <rdfs:domain rdf:resource="http://example.org/onto/class/google_data_loss_prevention_deidentify_template"/>
    <rdfs:range rdf:resource="http://www.w3.org/2001/XMLSchema#string"/>
  </owl:DatatypeProperty>
  <owl:DatatypeProperty rdf:about="http://example.org/onto/prop/google_data_loss_prevention_deidentify_template_year">
    <rdfs:label>year</rdfs:label>
    <rdfs:comment>Year of the date. Must be from 1 to 9999, or 0 to specify a date without a year.</rdfs:comment>
    <rdfs:domain rdf:resource="http://example.org/onto/class/google_data_loss_prevention_deidentify_template"/>
    <rdfs:range rdf:resource="http://www.w3.org/2001/XMLSchema#string"/>
  </owl:DatatypeProperty>
  <owl:DatatypeProperty rdf:about="http://example.org/onto/prop/google_data_loss_prevention_deidentify_template_hours">
    <rdfs:label>hours</rdfs:label>
    <rdfs:comment>Hours of day in 24 hour format. Should be from 0 to 23. An API may choose to allow the value "24:00:00" for scenarios like business closing time.</rdfs:comment>
    <rdfs:domain rdf:resource="http://example.org/onto/class/google_data_loss_prevention_deidentify_template"/>
    <rdfs:range rdf:resource="http://www.w3.org/2001/XMLSchema#string"/>
  </owl:DatatypeProperty>
  <owl:DatatypeProperty rdf:about="http://example.org/onto/prop/google_data_loss_prevention_deidentify_template_minutes">
    <rdfs:label>minutes</rdfs:label>
    <rdfs:comment>Minutes of hour of day. Must be from 0 to 59.</rdfs:comment>
    <rdfs:domain rdf:resource="http://example.org/onto/class/google_data_loss_prevention_deidentify_template"/>
    <rdfs:range rdf:resource="http://www.w3.org/2001/XMLSchema#string"/>
  </owl:DatatypeProperty>
  <owl:DatatypeProperty rdf:about="http://example.org/onto/prop/google_data_loss_prevention_deidentify_template_nanos">
    <rdfs:label>nanos</rdfs:label>
    <rdfs:comment>Fractions of seconds in nanoseconds. Must be from 0 to 999,999,999.</rdfs:comment>
    <rdfs:domain rdf:resource="http://example.org/onto/class/google_data_loss_prevention_deidentify_template"/>
    <rdfs:range rdf:resource="http://www.w3.org/2001/XMLSchema#string"/>
  </owl:DatatypeProperty>
  <owl:DatatypeProperty rdf:about="http://example.org/onto/prop/google_data_loss_prevention_deidentify_template_seconds">
    <rdfs:label>seconds</rdfs:label>
    <rdfs:comment>Seconds of minutes of the time. Must normally be from 0 to 59. An API may allow the value 60 if it allows leap-seconds.</rdfs:comment>
    <rdfs:domain rdf:resource="http://example.org/onto/class/google_data_loss_prevention_deidentify_template"/>
    <rdfs:range rdf:resource="http://www.w3.org/2001/XMLSchema#string"/>
  </owl:DatatypeProperty>
  <owl:DatatypeProperty rdf:about="http://example.org/onto/prop/google_data_loss_prevention_deidentify_template_masking_character">
    <rdfs:label>masking_character</rdfs:label>
    <rdfs:comment>Character to use to mask the sensitive values—for example, * for an alphabetic string such as a name, or 0 for a numeric string
such as ZIP code or credit card number. This string must have a length of 1. If not supplied, this value defaults to * for
strings, and 0 for digits.</rdfs:comment>
    <rdfs:domain rdf:resource="http://example.org/onto/class/google_data_loss_prevention_deidentify_template"/>
    <rdfs:range rdf:resource="http://www.w3.org/2001/XMLSchema#string"/>
  </owl:DatatypeProperty>
  <owl:DatatypeProperty rdf:about="http://example.org/onto/prop/google_data_loss_prevention_deidentify_template_number_to_mask">
    <rdfs:label>number_to_mask</rdfs:label>
    <rdfs:comment>Number of characters to mask. If not set, all matching chars will be masked. Skipped characters do not count towards this tally.
If number_to_mask is negative, this denotes inverse masking. Cloud DLP masks all but a number of characters. For example, suppose you have the following values:
- 'masking_character' is *
- 'number_to_mask' is -4
- 'reverse_order' is false
- 'characters_to_ignore' includes -
- Input string is 1234-5678-9012-3456

The resulting de-identified string is ****-****-****-3456. Cloud DLP masks all but the last four characters. If reverseOrder is true, all but the first four characters are masked as 1234-****-****-****.</rdfs:comment>
    <rdfs:domain rdf:resource="http://example.org/onto/class/google_data_loss_prevention_deidentify_template"/>
    <rdfs:range rdf:resource="http://www.w3.org/2001/XMLSchema#string"/>
  </owl:DatatypeProperty>
  <owl:DatatypeProperty rdf:about="http://example.org/onto/prop/google_data_loss_prevention_deidentify_template_reverse_order">
    <rdfs:label>reverse_order</rdfs:label>
    <rdfs:comment>Mask characters in reverse order. For example, if masking_character is 0, number_to_mask is 14, and reverse_order is 'false', then the
input string '1234-5678-9012-3456' is masked as '00000000000000-3456'.</rdfs:comment>
    <rdfs:domain rdf:resource="http://example.org/onto/class/google_data_loss_prevention_deidentify_template"/>
    <rdfs:range rdf:resource="http://www.w3.org/2001/XMLSchema#string"/>
  </owl:DatatypeProperty>
  <owl:DatatypeProperty rdf:about="http://example.org/onto/prop/google_data_loss_prevention_deidentify_template_characters_to_skip">
    <rdfs:label>characters_to_skip</rdfs:label>
    <rdfs:comment>Characters to not transform when masking. Only one of this or 'common_characters_to_ignore' must be specified.</rdfs:comment>
    <rdfs:domain rdf:resource="http://example.org/onto/class/google_data_loss_prevention_deidentify_template"/>
    <rdfs:range rdf:resource="http://www.w3.org/2001/XMLSchema#string"/>
  </owl:DatatypeProperty>
  <owl:DatatypeProperty rdf:about="http://example.org/onto/prop/google_data_loss_prevention_deidentify_template_common_characters_to_ignore">
    <rdfs:label>common_characters_to_ignore</rdfs:label>
    <rdfs:comment>Common characters to not transform when masking. Useful to avoid removing punctuation. Only one of this or 'characters_to_skip' must be specified. Possible values: ["NUMERIC", "ALPHA_UPPER_CASE", "ALPHA_LOWER_CASE", "PUNCTUATION", "WHITESPACE"]</rdfs:comment>
    <rdfs:domain rdf:resource="http://example.org/onto/class/google_data_loss_prevention_deidentify_template"/>
    <rdfs:range rdf:resource="http://www.w3.org/2001/XMLSchema#string"/>
  </owl:DatatypeProperty>
  <owl:DatatypeProperty rdf:about="http://example.org/onto/prop/google_data_loss_prevention_deidentify_template_name">
    <rdfs:label>name</rdfs:label>
    <rdfs:comment>Name describing the field.</rdfs:comment>
    <rdfs:domain rdf:resource="http://example.org/onto/class/google_data_loss_prevention_deidentify_template"/>
    <rdfs:range rdf:resource="http://www.w3.org/2001/XMLSchema#string"/>
  </owl:DatatypeProperty>
  <owl:DatatypeProperty rdf:about="http://example.org/onto/prop/google_data_loss_prevention_deidentify_template_crypto_key_name">
    <rdfs:label>crypto_key_name</rdfs:label>
    <rdfs:comment>The resource name of the KMS CryptoKey to use for unwrapping.</rdfs:comment>
    <rdfs:domain rdf:resource="http://example.org/onto/class/google_data_loss_prevention_deidentify_template"/>
    <rdfs:range rdf:resource="http://www.w3.org/2001/XMLSchema#string"/>
  </owl:DatatypeProperty>
  <owl:DatatypeProperty rdf:about="http://example.org/onto/prop/google_data_loss_prevention_deidentify_template_wrapped_key">
    <rdfs:label>wrapped_key</rdfs:label>
    <rdfs:comment>The wrapped data crypto key.

A base64-encoded string.</rdfs:comment>
    <rdfs:domain rdf:resource="http://example.org/onto/class/google_data_loss_prevention_deidentify_template"/>
    <rdfs:range rdf:resource="http://www.w3.org/2001/XMLSchema#string"/>
  </owl:DatatypeProperty>
  <owl:DatatypeProperty rdf:about="http://example.org/onto/prop/google_data_loss_prevention_deidentify_template_name">
    <rdfs:label>name</rdfs:label>
    <rdfs:comment>Name of the key. This is an arbitrary string used to differentiate different keys. A unique key is generated per name: two separate 'TransientCryptoKey' protos share the same generated key if their names are the same. When the data crypto key is generated, this name is not used in any way (repeating the api call will result in a different key being generated).</rdfs:comment>
    <rdfs:domain rdf:resource="http://example.org/onto/class/google_data_loss_prevention_deidentify_template"/>
    <rdfs:range rdf:resource="http://www.w3.org/2001/XMLSchema#string"/>
  </owl:DatatypeProperty>
  <owl:DatatypeProperty rdf:about="http://example.org/onto/prop/google_data_loss_prevention_deidentify_template_key">
    <rdfs:label>key</rdfs:label>
    <rdfs:comment>A 128/192/256 bit key.

A base64-encoded string.</rdfs:comment>
    <rdfs:domain rdf:resource="http://example.org/onto/class/google_data_loss_prevention_deidentify_template"/>
    <rdfs:range rdf:resource="http://www.w3.org/2001/XMLSchema#string"/>
  </owl:DatatypeProperty>
  <owl:DatatypeProperty rdf:about="http://example.org/onto/prop/google_data_loss_prevention_deidentify_template_name">
    <rdfs:label>name</rdfs:label>
    <rdfs:comment>Name of the information type. Either a name of your choosing when creating a CustomInfoType, or one of the names listed at [https://cloud.google.com/dlp/docs/infotypes-reference](https://cloud.google.com/dlp/docs/infotypes-reference) when specifying a built-in type. When sending Cloud DLP results to Data Catalog, infoType names should conform to the pattern '[A-Za-z0-9$-_]{1,64}'.</rdfs:comment>
    <rdfs:domain rdf:resource="http://example.org/onto/class/google_data_loss_prevention_deidentify_template"/>
    <rdfs:range rdf:resource="http://www.w3.org/2001/XMLSchema#string"/>
  </owl:DatatypeProperty>
  <owl:DatatypeProperty rdf:about="http://example.org/onto/prop/google_data_loss_prevention_deidentify_template_version">
    <rdfs:label>version</rdfs:label>
    <rdfs:comment>Optional version name for this InfoType.</rdfs:comment>
    <rdfs:domain rdf:resource="http://example.org/onto/class/google_data_loss_prevention_deidentify_template"/>
    <rdfs:range rdf:resource="http://www.w3.org/2001/XMLSchema#string"/>
  </owl:DatatypeProperty>
  <owl:DatatypeProperty rdf:about="http://example.org/onto/prop/google_data_loss_prevention_deidentify_template_score">
    <rdfs:label>score</rdfs:label>
    <rdfs:comment>The sensitivity score applied to the resource. Possible values: ["SENSITIVITY_LOW", "SENSITIVITY_MODERATE", "SENSITIVITY_HIGH"]</rdfs:comment>
    <rdfs:domain rdf:resource="http://example.org/onto/class/google_data_loss_prevention_deidentify_template"/>
    <rdfs:range rdf:resource="http://www.w3.org/2001/XMLSchema#string"/>
  </owl:DatatypeProperty>
  <owl:DatatypeProperty rdf:about="http://example.org/onto/prop/google_data_loss_prevention_deidentify_template_crypto_key_name">
    <rdfs:label>crypto_key_name</rdfs:label>
    <rdfs:comment>The resource name of the KMS CryptoKey to use for unwrapping.</rdfs:comment>
    <rdfs:domain rdf:resource="http://example.org/onto/class/google_data_loss_prevention_deidentify_template"/>
    <rdfs:range rdf:resource="http://www.w3.org/2001/XMLSchema#string"/>
  </owl:DatatypeProperty>
  <owl:DatatypeProperty rdf:about="http://example.org/onto/prop/google_data_loss_prevention_deidentify_template_wrapped_key">
    <rdfs:label>wrapped_key</rdfs:label>
    <rdfs:comment>The wrapped data crypto key.

A base64-encoded string.</rdfs:comment>
    <rdfs:domain rdf:resource="http://example.org/onto/class/google_data_loss_prevention_deidentify_template"/>
    <rdfs:range rdf:resource="http://www.w3.org/2001/XMLSchema#string"/>
  </owl:DatatypeProperty>
  <owl:DatatypeProperty rdf:about="http://example.org/onto/prop/google_data_loss_prevention_deidentify_template_name">
    <rdfs:label>name</rdfs:label>
    <rdfs:comment>Name of the key. This is an arbitrary string used to differentiate different keys. A unique key is generated per name: two separate 'TransientCryptoKey' protos share the same generated key if their names are the same. When the data crypto key is generated, this name is not used in any way (repeating the api call will result in a different key being generated).</rdfs:comment>
    <rdfs:domain rdf:resource="http://example.org/onto/class/google_data_loss_prevention_deidentify_template"/>
    <rdfs:range rdf:resource="http://www.w3.org/2001/XMLSchema#string"/>
  </owl:DatatypeProperty>
  <owl:DatatypeProperty rdf:about="http://example.org/onto/prop/google_data_loss_prevention_deidentify_template_key">
    <rdfs:label>key</rdfs:label>
    <rdfs:comment>A 128/192/256 bit key.

A base64-encoded string.</rdfs:comment>
    <rdfs:domain rdf:resource="http://example.org/onto/class/google_data_loss_prevention_deidentify_template"/>
    <rdfs:range rdf:resource="http://www.w3.org/2001/XMLSchema#string"/>
  </owl:DatatypeProperty>
  <owl:DatatypeProperty rdf:about="http://example.org/onto/prop/google_data_loss_prevention_deidentify_template_common_alphabet">
    <rdfs:label>common_alphabet</rdfs:label>
    <rdfs:comment>Common alphabets. Only one of this, 'custom_alphabet' or 'radix' must be specified. Possible values: ["NUMERIC", "HEXADECIMAL", "UPPER_CASE_ALPHA_NUMERIC", "ALPHA_NUMERIC"]</rdfs:comment>
    <rdfs:domain rdf:resource="http://example.org/onto/class/google_data_loss_prevention_deidentify_template"/>
    <rdfs:range rdf:resource="http://www.w3.org/2001/XMLSchema#string"/>
  </owl:DatatypeProperty>
  <owl:DatatypeProperty rdf:about="http://example.org/onto/prop/google_data_loss_prevention_deidentify_template_custom_alphabet">
    <rdfs:label>custom_alphabet</rdfs:label>
    <rdfs:comment>This is supported by mapping these to the alphanumeric characters that the FFX mode natively supports. This happens before/after encryption/decryption. Each character listed must appear only once. Number of characters must be in the range \[2, 95\]. This must be encoded as ASCII. The order of characters does not matter. The full list of allowed characters is:

''0123456789ABCDEFGHIJKLMNOPQRSTUVWXYZabcdefghijklmnopqrstuvwxyz ~'!@#$%^&*()_-+={[}]|:;"'<,>.?/''. Only one of this, 'common_alphabet' or 'radix' must be specified.</rdfs:comment>
    <rdfs:domain rdf:resource="http://example.org/onto/class/google_data_loss_prevention_deidentify_template"/>
    <rdfs:range rdf:resource="http://www.w3.org/2001/XMLSchema#string"/>
  </owl:DatatypeProperty>
  <owl:DatatypeProperty rdf:about="http://example.org/onto/prop/google_data_loss_prevention_deidentify_template_radix">
    <rdfs:label>radix</rdfs:label>
    <rdfs:comment>The native way to select the alphabet. Must be in the range \[2, 95\]. Only one of this, 'custom_alphabet' or 'common_alphabet' must be specified.</rdfs:comment>
    <rdfs:domain rdf:resource="http://example.org/onto/class/google_data_loss_prevention_deidentify_template"/>
    <rdfs:range rdf:resource="http://www.w3.org/2001/XMLSchema#string"/>
  </owl:DatatypeProperty>
  <owl:DatatypeProperty rdf:about="http://example.org/onto/prop/google_data_loss_prevention_deidentify_template_name">
    <rdfs:label>name</rdfs:label>
    <rdfs:comment>Name describing the field.</rdfs:comment>
    <rdfs:domain rdf:resource="http://example.org/onto/class/google_data_loss_prevention_deidentify_template"/>
    <rdfs:range rdf:resource="http://www.w3.org/2001/XMLSchema#string"/>
  </owl:DatatypeProperty>
  <owl:DatatypeProperty rdf:about="http://example.org/onto/prop/google_data_loss_prevention_deidentify_template_crypto_key_name">
    <rdfs:label>crypto_key_name</rdfs:label>
    <rdfs:comment>The resource name of the KMS CryptoKey to use for unwrapping.</rdfs:comment>
    <rdfs:domain rdf:resource="http://example.org/onto/class/google_data_loss_prevention_deidentify_template"/>
    <rdfs:range rdf:resource="http://www.w3.org/2001/XMLSchema#string"/>
  </owl:DatatypeProperty>
  <owl:DatatypeProperty rdf:about="http://example.org/onto/prop/google_data_loss_prevention_deidentify_template_wrapped_key">
    <rdfs:label>wrapped_key</rdfs:label>
    <rdfs:comment>The wrapped data crypto key.

A base64-encoded string.</rdfs:comment>
    <rdfs:domain rdf:resource="http://example.org/onto/class/google_data_loss_prevention_deidentify_template"/>
    <rdfs:range rdf:resource="http://www.w3.org/2001/XMLSchema#string"/>
  </owl:DatatypeProperty>
  <owl:DatatypeProperty rdf:about="http://example.org/onto/prop/google_data_loss_prevention_deidentify_template_name">
    <rdfs:label>name</rdfs:label>
    <rdfs:comment>Name of the key. This is an arbitrary string used to differentiate different keys. A unique key is generated per name: two separate 'TransientCryptoKey' protos share the same generated key if their names are the same. When the data crypto key is generated, this name is not used in any way (repeating the api call will result in a different key being generated).</rdfs:comment>
    <rdfs:domain rdf:resource="http://example.org/onto/class/google_data_loss_prevention_deidentify_template"/>
    <rdfs:range rdf:resource="http://www.w3.org/2001/XMLSchema#string"/>
  </owl:DatatypeProperty>
  <owl:DatatypeProperty rdf:about="http://example.org/onto/prop/google_data_loss_prevention_deidentify_template_key">
    <rdfs:label>key</rdfs:label>
    <rdfs:comment>A 128/192/256 bit key.

A base64-encoded string.</rdfs:comment>
    <rdfs:domain rdf:resource="http://example.org/onto/class/google_data_loss_prevention_deidentify_template"/>
    <rdfs:range rdf:resource="http://www.w3.org/2001/XMLSchema#string"/>
  </owl:DatatypeProperty>
  <owl:DatatypeProperty rdf:about="http://example.org/onto/prop/google_data_loss_prevention_deidentify_template_name">
    <rdfs:label>name</rdfs:label>
    <rdfs:comment>Name of the information type. Either a name of your choosing when creating a CustomInfoType, or one of the names listed at [https://cloud.google.com/dlp/docs/infotypes-reference](https://cloud.google.com/dlp/docs/infotypes-reference) when specifying a built-in type. When sending Cloud DLP results to Data Catalog, infoType names should conform to the pattern '[A-Za-z0-9$-_]{1,64}'.</rdfs:comment>
    <rdfs:domain rdf:resource="http://example.org/onto/class/google_data_loss_prevention_deidentify_template"/>
    <rdfs:range rdf:resource="http://www.w3.org/2001/XMLSchema#string"/>
  </owl:DatatypeProperty>
  <owl:DatatypeProperty rdf:about="http://example.org/onto/prop/google_data_loss_prevention_deidentify_template_version">
    <rdfs:label>version</rdfs:label>
    <rdfs:comment>Optional version name for this InfoType.</rdfs:comment>
    <rdfs:domain rdf:resource="http://example.org/onto/class/google_data_loss_prevention_deidentify_template"/>
    <rdfs:range rdf:resource="http://www.w3.org/2001/XMLSchema#string"/>
  </owl:DatatypeProperty>
  <owl:DatatypeProperty rdf:about="http://example.org/onto/prop/google_data_loss_prevention_deidentify_template_score">
    <rdfs:label>score</rdfs:label>
    <rdfs:comment>The sensitivity score applied to the resource. Possible values: ["SENSITIVITY_LOW", "SENSITIVITY_MODERATE", "SENSITIVITY_HIGH"]</rdfs:comment>
    <rdfs:domain rdf:resource="http://example.org/onto/class/google_data_loss_prevention_deidentify_template"/>
    <rdfs:range rdf:resource="http://www.w3.org/2001/XMLSchema#string"/>
  </owl:DatatypeProperty>
  <owl:DatatypeProperty rdf:about="http://example.org/onto/prop/google_data_loss_prevention_deidentify_template_lower_bound_days">
    <rdfs:label>lower_bound_days</rdfs:label>
    <rdfs:comment>For example, -5 means shift date to at most 5 days back in the past.</rdfs:comment>
    <rdfs:domain rdf:resource="http://example.org/onto/class/google_data_loss_prevention_deidentify_template"/>
    <rdfs:range rdf:resource="http://www.w3.org/2001/XMLSchema#string"/>
  </owl:DatatypeProperty>
  <owl:DatatypeProperty rdf:about="http://example.org/onto/prop/google_data_loss_prevention_deidentify_template_upper_bound_days">
    <rdfs:label>upper_bound_days</rdfs:label>
    <rdfs:comment>Range of shift in days. Actual shift will be selected at random within this range (inclusive ends). Negative means shift to earlier in time. Must not be more than 365250 days (1000 years) each direction.

For example, 3 means shift date to at most 3 days into the future.</rdfs:comment>
    <rdfs:domain rdf:resource="http://example.org/onto/class/google_data_loss_prevention_deidentify_template"/>
    <rdfs:range rdf:resource="http://www.w3.org/2001/XMLSchema#string"/>
  </owl:DatatypeProperty>
  <owl:DatatypeProperty rdf:about="http://example.org/onto/prop/google_data_loss_prevention_deidentify_template_name">
    <rdfs:label>name</rdfs:label>
    <rdfs:comment>Name describing the field.</rdfs:comment>
    <rdfs:domain rdf:resource="http://example.org/onto/class/google_data_loss_prevention_deidentify_template"/>
    <rdfs:range rdf:resource="http://www.w3.org/2001/XMLSchema#string"/>
  </owl:DatatypeProperty>
  <owl:DatatypeProperty rdf:about="http://example.org/onto/prop/google_data_loss_prevention_deidentify_template_crypto_key_name">
    <rdfs:label>crypto_key_name</rdfs:label>
    <rdfs:comment>The resource name of the KMS CryptoKey to use for unwrapping.</rdfs:comment>
    <rdfs:domain rdf:resource="http://example.org/onto/class/google_data_loss_prevention_deidentify_template"/>
    <rdfs:range rdf:resource="http://www.w3.org/2001/XMLSchema#string"/>
  </owl:DatatypeProperty>
  <owl:DatatypeProperty rdf:about="http://example.org/onto/prop/google_data_loss_prevention_deidentify_template_wrapped_key">
    <rdfs:label>wrapped_key</rdfs:label>
    <rdfs:comment>The wrapped data crypto key.

A base64-encoded string.</rdfs:comment>
    <rdfs:domain rdf:resource="http://example.org/onto/class/google_data_loss_prevention_deidentify_template"/>
    <rdfs:range rdf:resource="http://www.w3.org/2001/XMLSchema#string"/>
  </owl:DatatypeProperty>
  <owl:DatatypeProperty rdf:about="http://example.org/onto/prop/google_data_loss_prevention_deidentify_template_name">
    <rdfs:label>name</rdfs:label>
    <rdfs:comment>Name of the key. This is an arbitrary string used to differentiate different keys. A unique key is generated per name: two separate 'TransientCryptoKey' protos share the same generated key if their names are the same. When the data crypto key is generated, this name is not used in any way (repeating the api call will result in a different key being generated).</rdfs:comment>
    <rdfs:domain rdf:resource="http://example.org/onto/class/google_data_loss_prevention_deidentify_template"/>
    <rdfs:range rdf:resource="http://www.w3.org/2001/XMLSchema#string"/>
  </owl:DatatypeProperty>
  <owl:DatatypeProperty rdf:about="http://example.org/onto/prop/google_data_loss_prevention_deidentify_template_key">
    <rdfs:label>key</rdfs:label>
    <rdfs:comment>A 128/192/256 bit key.

A base64-encoded string.</rdfs:comment>
    <rdfs:domain rdf:resource="http://example.org/onto/class/google_data_loss_prevention_deidentify_template"/>
    <rdfs:range rdf:resource="http://www.w3.org/2001/XMLSchema#string"/>
  </owl:DatatypeProperty>
  <owl:DatatypeProperty rdf:about="http://example.org/onto/prop/google_data_loss_prevention_deidentify_template_bucket_size">
    <rdfs:label>bucket_size</rdfs:label>
    <rdfs:comment>Size of each bucket (except for minimum and maximum buckets).
So if lower_bound = 10, upper_bound = 89, and bucketSize = 10, then the following buckets would be used: -10, 10-20, 20-30, 30-40, 40-50, 50-60, 60-70, 70-80, 80-89, 89+.
Precision up to 2 decimals works.</rdfs:comment>
    <rdfs:domain rdf:resource="http://example.org/onto/class/google_data_loss_prevention_deidentify_template"/>
    <rdfs:range rdf:resource="http://www.w3.org/2001/XMLSchema#string"/>
  </owl:DatatypeProperty>
  <owl:DatatypeProperty rdf:about="http://example.org/onto/prop/google_data_loss_prevention_deidentify_template_float_value">
    <rdfs:label>float_value</rdfs:label>
    <rdfs:comment>A float value.</rdfs:comment>
    <rdfs:domain rdf:resource="http://example.org/onto/class/google_data_loss_prevention_deidentify_template"/>
    <rdfs:range rdf:resource="http://www.w3.org/2001/XMLSchema#string"/>
  </owl:DatatypeProperty>
  <owl:DatatypeProperty rdf:about="http://example.org/onto/prop/google_data_loss_prevention_deidentify_template_integer_value">
    <rdfs:label>integer_value</rdfs:label>
    <rdfs:comment>An integer value (int64 format)</rdfs:comment>
    <rdfs:domain rdf:resource="http://example.org/onto/class/google_data_loss_prevention_deidentify_template"/>
    <rdfs:range rdf:resource="http://www.w3.org/2001/XMLSchema#string"/>
  </owl:DatatypeProperty>
  <owl:DatatypeProperty rdf:about="http://example.org/onto/prop/google_data_loss_prevention_deidentify_template_float_value">
    <rdfs:label>float_value</rdfs:label>
    <rdfs:comment>A float value.</rdfs:comment>
    <rdfs:domain rdf:resource="http://example.org/onto/class/google_data_loss_prevention_deidentify_template"/>
    <rdfs:range rdf:resource="http://www.w3.org/2001/XMLSchema#string"/>
  </owl:DatatypeProperty>
  <owl:DatatypeProperty rdf:about="http://example.org/onto/prop/google_data_loss_prevention_deidentify_template_integer_value">
    <rdfs:label>integer_value</rdfs:label>
    <rdfs:comment>An integer value (int64 format)</rdfs:comment>
    <rdfs:domain rdf:resource="http://example.org/onto/class/google_data_loss_prevention_deidentify_template"/>
    <rdfs:range rdf:resource="http://www.w3.org/2001/XMLSchema#string"/>
  </owl:DatatypeProperty>
  <owl:DatatypeProperty rdf:about="http://example.org/onto/prop/google_data_loss_prevention_deidentify_template_boolean_value">
    <rdfs:label>boolean_value</rdfs:label>
    <rdfs:comment>A boolean value.</rdfs:comment>
    <rdfs:domain rdf:resource="http://example.org/onto/class/google_data_loss_prevention_deidentify_template"/>
    <rdfs:range rdf:resource="http://www.w3.org/2001/XMLSchema#string"/>
  </owl:DatatypeProperty>
  <owl:DatatypeProperty rdf:about="http://example.org/onto/prop/google_data_loss_prevention_deidentify_template_day_of_week_value">
    <rdfs:label>day_of_week_value</rdfs:label>
    <rdfs:comment>Represents a day of the week. Possible values: ["MONDAY", "TUESDAY", "WEDNESDAY", "THURSDAY", "FRIDAY", "SATURDAY", "SUNDAY"]</rdfs:comment>
    <rdfs:domain rdf:resource="http://example.org/onto/class/google_data_loss_prevention_deidentify_template"/>
    <rdfs:range rdf:resource="http://www.w3.org/2001/XMLSchema#string"/>
  </owl:DatatypeProperty>
  <owl:DatatypeProperty rdf:about="http://example.org/onto/prop/google_data_loss_prevention_deidentify_template_float_value">
    <rdfs:label>float_value</rdfs:label>
    <rdfs:comment>A float value.</rdfs:comment>
    <rdfs:domain rdf:resource="http://example.org/onto/class/google_data_loss_prevention_deidentify_template"/>
    <rdfs:range rdf:resource="http://www.w3.org/2001/XMLSchema#string"/>
  </owl:DatatypeProperty>
  <owl:DatatypeProperty rdf:about="http://example.org/onto/prop/google_data_loss_prevention_deidentify_template_integer_value">
    <rdfs:label>integer_value</rdfs:label>
    <rdfs:comment>An integer value (int64 format)</rdfs:comment>
    <rdfs:domain rdf:resource="http://example.org/onto/class/google_data_loss_prevention_deidentify_template"/>
    <rdfs:range rdf:resource="http://www.w3.org/2001/XMLSchema#string"/>
  </owl:DatatypeProperty>
  <owl:DatatypeProperty rdf:about="http://example.org/onto/prop/google_data_loss_prevention_deidentify_template_string_value">
    <rdfs:label>string_value</rdfs:label>
    <rdfs:comment>A string value.</rdfs:comment>
    <rdfs:domain rdf:resource="http://example.org/onto/class/google_data_loss_prevention_deidentify_template"/>
    <rdfs:range rdf:resource="http://www.w3.org/2001/XMLSchema#string"/>
  </owl:DatatypeProperty>
  <owl:DatatypeProperty rdf:about="http://example.org/onto/prop/google_data_loss_prevention_deidentify_template_timestamp_value">
    <rdfs:label>timestamp_value</rdfs:label>
    <rdfs:comment>A timestamp in RFC3339 UTC "Zulu" format, with nanosecond resolution and up to nine fractional digits.
Examples: "2014-10-02T15:01:23Z" and "2014-10-02T15:01:23.045123456Z".</rdfs:comment>
    <rdfs:domain rdf:resource="http://example.org/onto/class/google_data_loss_prevention_deidentify_template"/>
    <rdfs:range rdf:resource="http://www.w3.org/2001/XMLSchema#string"/>
  </owl:DatatypeProperty>
  <owl:DatatypeProperty rdf:about="http://example.org/onto/prop/google_data_loss_prevention_deidentify_template_day">
    <rdfs:label>day</rdfs:label>
    <rdfs:comment>Day of a month. Must be from 1 to 31 and valid for the year and month, or 0 to specify a year by itself or a year and month where the day isn't significant.</rdfs:comment>
    <rdfs:domain rdf:resource="http://example.org/onto/class/google_data_loss_prevention_deidentify_template"/>
    <rdfs:range rdf:resource="http://www.w3.org/2001/XMLSchema#string"/>
  </owl:DatatypeProperty>
  <owl:DatatypeProperty rdf:about="http://example.org/onto/prop/google_data_loss_prevention_deidentify_template_month">
    <rdfs:label>month</rdfs:label>
    <rdfs:comment>Month of a year. Must be from 1 to 12, or 0 to specify a year without a month and day.</rdfs:comment>
    <rdfs:domain rdf:resource="http://example.org/onto/class/google_data_loss_prevention_deidentify_template"/>
    <rdfs:range rdf:resource="http://www.w3.org/2001/XMLSchema#string"/>
  </owl:DatatypeProperty>
  <owl:DatatypeProperty rdf:about="http://example.org/onto/prop/google_data_loss_prevention_deidentify_template_year">
    <rdfs:label>year</rdfs:label>
    <rdfs:comment>Year of the date. Must be from 1 to 9999, or 0 to specify a date without a year.</rdfs:comment>
    <rdfs:domain rdf:resource="http://example.org/onto/class/google_data_loss_prevention_deidentify_template"/>
    <rdfs:range rdf:resource="http://www.w3.org/2001/XMLSchema#string"/>
  </owl:DatatypeProperty>
  <owl:DatatypeProperty rdf:about="http://example.org/onto/prop/google_data_loss_prevention_deidentify_template_hours">
    <rdfs:label>hours</rdfs:label>
    <rdfs:comment>Hours of day in 24 hour format. Should be from 0 to 23. An API may choose to allow the value "24:00:00" for scenarios like business closing time.</rdfs:comment>
    <rdfs:domain rdf:resource="http://example.org/onto/class/google_data_loss_prevention_deidentify_template"/>
    <rdfs:range rdf:resource="http://www.w3.org/2001/XMLSchema#string"/>
  </owl:DatatypeProperty>
  <owl:DatatypeProperty rdf:about="http://example.org/onto/prop/google_data_loss_prevention_deidentify_template_minutes">
    <rdfs:label>minutes</rdfs:label>
    <rdfs:comment>Minutes of hour of day. Must be from 0 to 59.</rdfs:comment>
    <rdfs:domain rdf:resource="http://example.org/onto/class/google_data_loss_prevention_deidentify_template"/>
    <rdfs:range rdf:resource="http://www.w3.org/2001/XMLSchema#string"/>
  </owl:DatatypeProperty>
  <owl:DatatypeProperty rdf:about="http://example.org/onto/prop/google_data_loss_prevention_deidentify_template_nanos">
    <rdfs:label>nanos</rdfs:label>
    <rdfs:comment>Fractions of seconds in nanoseconds. Must be from 0 to 999,999,999.</rdfs:comment>
    <rdfs:domain rdf:resource="http://example.org/onto/class/google_data_loss_prevention_deidentify_template"/>
    <rdfs:range rdf:resource="http://www.w3.org/2001/XMLSchema#string"/>
  </owl:DatatypeProperty>
  <owl:DatatypeProperty rdf:about="http://example.org/onto/prop/google_data_loss_prevention_deidentify_template_seconds">
    <rdfs:label>seconds</rdfs:label>
    <rdfs:comment>Seconds of minutes of the time. Must normally be from 0 to 59. An API may allow the value 60 if it allows leap-seconds.</rdfs:comment>
    <rdfs:domain rdf:resource="http://example.org/onto/class/google_data_loss_prevention_deidentify_template"/>
    <rdfs:range rdf:resource="http://www.w3.org/2001/XMLSchema#string"/>
  </owl:DatatypeProperty>
  <owl:DatatypeProperty rdf:about="http://example.org/onto/prop/google_data_loss_prevention_deidentify_template_words">
    <rdfs:label>words</rdfs:label>
    <rdfs:comment>Words or phrases defining the dictionary. The dictionary must contain at least one phrase and every phrase must contain at least 2 characters that are letters or digits.</rdfs:comment>
    <rdfs:domain rdf:resource="http://example.org/onto/class/google_data_loss_prevention_deidentify_template"/>
    <rdfs:range rdf:resource="http://www.w3.org/2001/XMLSchema#string"/>
  </owl:DatatypeProperty>
  <owl:DatatypeProperty rdf:about="http://example.org/onto/prop/google_data_loss_prevention_deidentify_template_part_to_extract">
    <rdfs:label>part_to_extract</rdfs:label>
    <rdfs:comment>The part of the time to keep. Possible values: ["YEAR", "MONTH", "DAY_OF_MONTH", "DAY_OF_WEEK", "WEEK_OF_YEAR", "HOUR_OF_DAY"]</rdfs:comment>
    <rdfs:domain rdf:resource="http://example.org/onto/class/google_data_loss_prevention_deidentify_template"/>
    <rdfs:range rdf:resource="http://www.w3.org/2001/XMLSchema#string"/>
  </owl:DatatypeProperty>
  <owl:DatatypeProperty rdf:about="http://example.org/onto/prop/google_data_loss_prevention_deidentify_template_boolean_value">
    <rdfs:label>boolean_value</rdfs:label>
    <rdfs:comment>A boolean value.</rdfs:comment>
    <rdfs:domain rdf:resource="http://example.org/onto/class/google_data_loss_prevention_deidentify_template"/>
    <rdfs:range rdf:resource="http://www.w3.org/2001/XMLSchema#string"/>
  </owl:DatatypeProperty>
  <owl:DatatypeProperty rdf:about="http://example.org/onto/prop/google_data_loss_prevention_deidentify_template_day_of_week_value">
    <rdfs:label>day_of_week_value</rdfs:label>
    <rdfs:comment>Represents a day of the week. Possible values: ["MONDAY", "TUESDAY", "WEDNESDAY", "THURSDAY", "FRIDAY", "SATURDAY", "SUNDAY"]</rdfs:comment>
    <rdfs:domain rdf:resource="http://example.org/onto/class/google_data_loss_prevention_deidentify_template"/>
    <rdfs:range rdf:resource="http://www.w3.org/2001/XMLSchema#string"/>
  </owl:DatatypeProperty>
  <owl:DatatypeProperty rdf:about="http://example.org/onto/prop/google_data_loss_prevention_deidentify_template_float_value">
    <rdfs:label>float_value</rdfs:label>
    <rdfs:comment>A float value.</rdfs:comment>
    <rdfs:domain rdf:resource="http://example.org/onto/class/google_data_loss_prevention_deidentify_template"/>
    <rdfs:range rdf:resource="http://www.w3.org/2001/XMLSchema#string"/>
  </owl:DatatypeProperty>
  <owl:DatatypeProperty rdf:about="http://example.org/onto/prop/google_data_loss_prevention_deidentify_template_integer_value">
    <rdfs:label>integer_value</rdfs:label>
    <rdfs:comment>An integer value (int64 format)</rdfs:comment>
    <rdfs:domain rdf:resource="http://example.org/onto/class/google_data_loss_prevention_deidentify_template"/>
    <rdfs:range rdf:resource="http://www.w3.org/2001/XMLSchema#string"/>
  </owl:DatatypeProperty>
  <owl:DatatypeProperty rdf:about="http://example.org/onto/prop/google_data_loss_prevention_deidentify_template_string_value">
    <rdfs:label>string_value</rdfs:label>
    <rdfs:comment>A string value.</rdfs:comment>
    <rdfs:domain rdf:resource="http://example.org/onto/class/google_data_loss_prevention_deidentify_template"/>
    <rdfs:range rdf:resource="http://www.w3.org/2001/XMLSchema#string"/>
  </owl:DatatypeProperty>
  <owl:DatatypeProperty rdf:about="http://example.org/onto/prop/google_data_loss_prevention_deidentify_template_timestamp_value">
    <rdfs:label>timestamp_value</rdfs:label>
    <rdfs:comment>A timestamp in RFC3339 UTC "Zulu" format, with nanosecond resolution and up to nine fractional digits. Examples: "2014-10-02T15:01:23Z" and "2014-10-02T15:01:23.045123456Z".</rdfs:comment>
    <rdfs:domain rdf:resource="http://example.org/onto/class/google_data_loss_prevention_deidentify_template"/>
    <rdfs:range rdf:resource="http://www.w3.org/2001/XMLSchema#string"/>
  </owl:DatatypeProperty>
  <owl:DatatypeProperty rdf:about="http://example.org/onto/prop/google_data_loss_prevention_deidentify_template_day">
    <rdfs:label>day</rdfs:label>
    <rdfs:comment>Day of a month. Must be from 1 to 31 and valid for the year and month, or 0 to specify a year by itself or a year and month where the day isn't significant.</rdfs:comment>
    <rdfs:domain rdf:resource="http://example.org/onto/class/google_data_loss_prevention_deidentify_template"/>
    <rdfs:range rdf:resource="http://www.w3.org/2001/XMLSchema#string"/>
  </owl:DatatypeProperty>
  <owl:DatatypeProperty rdf:about="http://example.org/onto/prop/google_data_loss_prevention_deidentify_template_month">
    <rdfs:label>month</rdfs:label>
    <rdfs:comment>Month of a year. Must be from 1 to 12, or 0 to specify a year without a month and day.</rdfs:comment>
    <rdfs:domain rdf:resource="http://example.org/onto/class/google_data_loss_prevention_deidentify_template"/>
    <rdfs:range rdf:resource="http://www.w3.org/2001/XMLSchema#string"/>
  </owl:DatatypeProperty>
  <owl:DatatypeProperty rdf:about="http://example.org/onto/prop/google_data_loss_prevention_deidentify_template_year">
    <rdfs:label>year</rdfs:label>
    <rdfs:comment>Year of the date. Must be from 1 to 9999, or 0 to specify a date without a year.</rdfs:comment>
    <rdfs:domain rdf:resource="http://example.org/onto/class/google_data_loss_prevention_deidentify_template"/>
    <rdfs:range rdf:resource="http://www.w3.org/2001/XMLSchema#string"/>
  </owl:DatatypeProperty>
  <owl:DatatypeProperty rdf:about="http://example.org/onto/prop/google_data_loss_prevention_deidentify_template_hours">
    <rdfs:label>hours</rdfs:label>
    <rdfs:comment>Hours of day in 24 hour format. Should be from 0 to 23. An API may choose to allow the value "24:00:00" for scenarios like business closing time.</rdfs:comment>
    <rdfs:domain rdf:resource="http://example.org/onto/class/google_data_loss_prevention_deidentify_template"/>
    <rdfs:range rdf:resource="http://www.w3.org/2001/XMLSchema#string"/>
  </owl:DatatypeProperty>
  <owl:DatatypeProperty rdf:about="http://example.org/onto/prop/google_data_loss_prevention_deidentify_template_minutes">
    <rdfs:label>minutes</rdfs:label>
    <rdfs:comment>Minutes of hour of day. Must be from 0 to 59.</rdfs:comment>
    <rdfs:domain rdf:resource="http://example.org/onto/class/google_data_loss_prevention_deidentify_template"/>
    <rdfs:range rdf:resource="http://www.w3.org/2001/XMLSchema#string"/>
  </owl:DatatypeProperty>
  <owl:DatatypeProperty rdf:about="http://example.org/onto/prop/google_data_loss_prevention_deidentify_template_nanos">
    <rdfs:label>nanos</rdfs:label>
    <rdfs:comment>Fractions of seconds in nanoseconds. Must be from 0 to 999,999,999.</rdfs:comment>
    <rdfs:domain rdf:resource="http://example.org/onto/class/google_data_loss_prevention_deidentify_template"/>
    <rdfs:range rdf:resource="http://www.w3.org/2001/XMLSchema#string"/>
  </owl:DatatypeProperty>
  <owl:DatatypeProperty rdf:about="http://example.org/onto/prop/google_data_loss_prevention_deidentify_template_seconds">
    <rdfs:label>seconds</rdfs:label>
    <rdfs:comment>Seconds of minutes of the time. Must normally be from 0 to 59. An API may allow the value 60 if it allows leap-seconds.</rdfs:comment>
    <rdfs:domain rdf:resource="http://example.org/onto/class/google_data_loss_prevention_deidentify_template"/>
    <rdfs:range rdf:resource="http://www.w3.org/2001/XMLSchema#string"/>
  </owl:DatatypeProperty>
  <owl:DatatypeProperty rdf:about="http://example.org/onto/prop/google_data_loss_prevention_deidentify_template_boolean_value">
    <rdfs:label>boolean_value</rdfs:label>
    <rdfs:comment>A boolean value.</rdfs:comment>
    <rdfs:domain rdf:resource="http://example.org/onto/class/google_data_loss_prevention_deidentify_template"/>
    <rdfs:range rdf:resource="http://www.w3.org/2001/XMLSchema#string"/>
  </owl:DatatypeProperty>
  <owl:DatatypeProperty rdf:about="http://example.org/onto/prop/google_data_loss_prevention_deidentify_template_day_of_week_value">
    <rdfs:label>day_of_week_value</rdfs:label>
    <rdfs:comment>Represents a day of the week. Possible values: ["MONDAY", "TUESDAY", "WEDNESDAY", "THURSDAY", "FRIDAY", "SATURDAY", "SUNDAY"]</rdfs:comment>
    <rdfs:domain rdf:resource="http://example.org/onto/class/google_data_loss_prevention_deidentify_template"/>
    <rdfs:range rdf:resource="http://www.w3.org/2001/XMLSchema#string"/>
  </owl:DatatypeProperty>
  <owl:DatatypeProperty rdf:about="http://example.org/onto/prop/google_data_loss_prevention_deidentify_template_float_value">
    <rdfs:label>float_value</rdfs:label>
    <rdfs:comment>A float value.</rdfs:comment>
    <rdfs:domain rdf:resource="http://example.org/onto/class/google_data_loss_prevention_deidentify_template"/>
    <rdfs:range rdf:resource="http://www.w3.org/2001/XMLSchema#string"/>
  </owl:DatatypeProperty>
  <owl:DatatypeProperty rdf:about="http://example.org/onto/prop/google_data_loss_prevention_deidentify_template_integer_value">
    <rdfs:label>integer_value</rdfs:label>
    <rdfs:comment>An integer value (int64 format)</rdfs:comment>
    <rdfs:domain rdf:resource="http://example.org/onto/class/google_data_loss_prevention_deidentify_template"/>
    <rdfs:range rdf:resource="http://www.w3.org/2001/XMLSchema#string"/>
  </owl:DatatypeProperty>
  <owl:DatatypeProperty rdf:about="http://example.org/onto/prop/google_data_loss_prevention_deidentify_template_string_value">
    <rdfs:label>string_value</rdfs:label>
    <rdfs:comment>A string value.</rdfs:comment>
    <rdfs:domain rdf:resource="http://example.org/onto/class/google_data_loss_prevention_deidentify_template"/>
    <rdfs:range rdf:resource="http://www.w3.org/2001/XMLSchema#string"/>
  </owl:DatatypeProperty>
  <owl:DatatypeProperty rdf:about="http://example.org/onto/prop/google_data_loss_prevention_deidentify_template_timestamp_value">
    <rdfs:label>timestamp_value</rdfs:label>
    <rdfs:comment>A timestamp in RFC3339 UTC "Zulu" format, with nanosecond resolution and up to nine fractional digits. Examples: "2014-10-02T15:01:23Z" and "2014-10-02T15:01:23.045123456Z".</rdfs:comment>
    <rdfs:domain rdf:resource="http://example.org/onto/class/google_data_loss_prevention_deidentify_template"/>
    <rdfs:range rdf:resource="http://www.w3.org/2001/XMLSchema#string"/>
  </owl:DatatypeProperty>
  <owl:DatatypeProperty rdf:about="http://example.org/onto/prop/google_data_loss_prevention_deidentify_template_day">
    <rdfs:label>day</rdfs:label>
    <rdfs:comment>Day of a month. Must be from 1 to 31 and valid for the year and month, or 0 to specify a year by itself or a year and month where the day isn't significant.</rdfs:comment>
    <rdfs:domain rdf:resource="http://example.org/onto/class/google_data_loss_prevention_deidentify_template"/>
    <rdfs:range rdf:resource="http://www.w3.org/2001/XMLSchema#string"/>
  </owl:DatatypeProperty>
  <owl:DatatypeProperty rdf:about="http://example.org/onto/prop/google_data_loss_prevention_deidentify_template_month">
    <rdfs:label>month</rdfs:label>
    <rdfs:comment>Month of a year. Must be from 1 to 12, or 0 to specify a year without a month and day.</rdfs:comment>
    <rdfs:domain rdf:resource="http://example.org/onto/class/google_data_loss_prevention_deidentify_template"/>
    <rdfs:range rdf:resource="http://www.w3.org/2001/XMLSchema#string"/>
  </owl:DatatypeProperty>
  <owl:DatatypeProperty rdf:about="http://example.org/onto/prop/google_data_loss_prevention_deidentify_template_year">
    <rdfs:label>year</rdfs:label>
    <rdfs:comment>Year of the date. Must be from 1 to 9999, or 0 to specify a date without a year.</rdfs:comment>
    <rdfs:domain rdf:resource="http://example.org/onto/class/google_data_loss_prevention_deidentify_template"/>
    <rdfs:range rdf:resource="http://www.w3.org/2001/XMLSchema#string"/>
  </owl:DatatypeProperty>
  <owl:DatatypeProperty rdf:about="http://example.org/onto/prop/google_data_loss_prevention_deidentify_template_hours">
    <rdfs:label>hours</rdfs:label>
    <rdfs:comment>Hours of day in 24 hour format. Should be from 0 to 23. An API may choose to allow the value "24:00:00" for scenarios like business closing time.</rdfs:comment>
    <rdfs:domain rdf:resource="http://example.org/onto/class/google_data_loss_prevention_deidentify_template"/>
    <rdfs:range rdf:resource="http://www.w3.org/2001/XMLSchema#string"/>
  </owl:DatatypeProperty>
  <owl:DatatypeProperty rdf:about="http://example.org/onto/prop/google_data_loss_prevention_deidentify_template_minutes">
    <rdfs:label>minutes</rdfs:label>
    <rdfs:comment>Minutes of hour of day. Must be from 0 to 59.</rdfs:comment>
    <rdfs:domain rdf:resource="http://example.org/onto/class/google_data_loss_prevention_deidentify_template"/>
    <rdfs:range rdf:resource="http://www.w3.org/2001/XMLSchema#string"/>
  </owl:DatatypeProperty>
  <owl:DatatypeProperty rdf:about="http://example.org/onto/prop/google_data_loss_prevention_deidentify_template_nanos">
    <rdfs:label>nanos</rdfs:label>
    <rdfs:comment>Fractions of seconds in nanoseconds. Must be from 0 to 999,999,999.</rdfs:comment>
    <rdfs:domain rdf:resource="http://example.org/onto/class/google_data_loss_prevention_deidentify_template"/>
    <rdfs:range rdf:resource="http://www.w3.org/2001/XMLSchema#string"/>
  </owl:DatatypeProperty>
  <owl:DatatypeProperty rdf:about="http://example.org/onto/prop/google_data_loss_prevention_deidentify_template_seconds">
    <rdfs:label>seconds</rdfs:label>
    <rdfs:comment>Seconds of minutes of the time. Must normally be from 0 to 59. An API may allow the value 60 if it allows leap-seconds.</rdfs:comment>
    <rdfs:domain rdf:resource="http://example.org/onto/class/google_data_loss_prevention_deidentify_template"/>
    <rdfs:range rdf:resource="http://www.w3.org/2001/XMLSchema#string"/>
  </owl:DatatypeProperty>
  <owl:DatatypeProperty rdf:about="http://example.org/onto/prop/google_data_loss_prevention_deidentify_template_boolean_value">
    <rdfs:label>boolean_value</rdfs:label>
    <rdfs:comment>A boolean value.</rdfs:comment>
    <rdfs:domain rdf:resource="http://example.org/onto/class/google_data_loss_prevention_deidentify_template"/>
    <rdfs:range rdf:resource="http://www.w3.org/2001/XMLSchema#string"/>
  </owl:DatatypeProperty>
  <owl:DatatypeProperty rdf:about="http://example.org/onto/prop/google_data_loss_prevention_deidentify_template_day_of_week_value">
    <rdfs:label>day_of_week_value</rdfs:label>
    <rdfs:comment>Represents a day of the week. Possible values: ["MONDAY", "TUESDAY", "WEDNESDAY", "THURSDAY", "FRIDAY", "SATURDAY", "SUNDAY"]</rdfs:comment>
    <rdfs:domain rdf:resource="http://example.org/onto/class/google_data_loss_prevention_deidentify_template"/>
    <rdfs:range rdf:resource="http://www.w3.org/2001/XMLSchema#string"/>
  </owl:DatatypeProperty>
  <owl:DatatypeProperty rdf:about="http://example.org/onto/prop/google_data_loss_prevention_deidentify_template_float_value">
    <rdfs:label>float_value</rdfs:label>
    <rdfs:comment>A float value.</rdfs:comment>
    <rdfs:domain rdf:resource="http://example.org/onto/class/google_data_loss_prevention_deidentify_template"/>
    <rdfs:range rdf:resource="http://www.w3.org/2001/XMLSchema#string"/>
  </owl:DatatypeProperty>
  <owl:DatatypeProperty rdf:about="http://example.org/onto/prop/google_data_loss_prevention_deidentify_template_integer_value">
    <rdfs:label>integer_value</rdfs:label>
    <rdfs:comment>An integer value (int64 format)</rdfs:comment>
    <rdfs:domain rdf:resource="http://example.org/onto/class/google_data_loss_prevention_deidentify_template"/>
    <rdfs:range rdf:resource="http://www.w3.org/2001/XMLSchema#string"/>
  </owl:DatatypeProperty>
  <owl:DatatypeProperty rdf:about="http://example.org/onto/prop/google_data_loss_prevention_deidentify_template_string_value">
    <rdfs:label>string_value</rdfs:label>
    <rdfs:comment>A string value.</rdfs:comment>
    <rdfs:domain rdf:resource="http://example.org/onto/class/google_data_loss_prevention_deidentify_template"/>
    <rdfs:range rdf:resource="http://www.w3.org/2001/XMLSchema#string"/>
  </owl:DatatypeProperty>
  <owl:DatatypeProperty rdf:about="http://example.org/onto/prop/google_data_loss_prevention_deidentify_template_timestamp_value">
    <rdfs:label>timestamp_value</rdfs:label>
    <rdfs:comment>A timestamp in RFC3339 UTC "Zulu" format, with nanosecond resolution and up to nine fractional digits. Examples: "2014-10-02T15:01:23Z" and "2014-10-02T15:01:23.045123456Z".</rdfs:comment>
    <rdfs:domain rdf:resource="http://example.org/onto/class/google_data_loss_prevention_deidentify_template"/>
    <rdfs:range rdf:resource="http://www.w3.org/2001/XMLSchema#string"/>
  </owl:DatatypeProperty>
  <owl:DatatypeProperty rdf:about="http://example.org/onto/prop/google_data_loss_prevention_deidentify_template_day">
    <rdfs:label>day</rdfs:label>
    <rdfs:comment>Day of a month. Must be from 1 to 31 and valid for the year and month, or 0 to specify a year by itself or a year and month where the day isn't significant.</rdfs:comment>
    <rdfs:domain rdf:resource="http://example.org/onto/class/google_data_loss_prevention_deidentify_template"/>
    <rdfs:range rdf:resource="http://www.w3.org/2001/XMLSchema#string"/>
  </owl:DatatypeProperty>
  <owl:DatatypeProperty rdf:about="http://example.org/onto/prop/google_data_loss_prevention_deidentify_template_month">
    <rdfs:label>month</rdfs:label>
    <rdfs:comment>Month of a year. Must be from 1 to 12, or 0 to specify a year without a month and day.</rdfs:comment>
    <rdfs:domain rdf:resource="http://example.org/onto/class/google_data_loss_prevention_deidentify_template"/>
    <rdfs:range rdf:resource="http://www.w3.org/2001/XMLSchema#string"/>
  </owl:DatatypeProperty>
  <owl:DatatypeProperty rdf:about="http://example.org/onto/prop/google_data_loss_prevention_deidentify_template_year">
    <rdfs:label>year</rdfs:label>
    <rdfs:comment>Year of the date. Must be from 1 to 9999, or 0 to specify a date without a year.</rdfs:comment>
    <rdfs:domain rdf:resource="http://example.org/onto/class/google_data_loss_prevention_deidentify_template"/>
    <rdfs:range rdf:resource="http://www.w3.org/2001/XMLSchema#string"/>
  </owl:DatatypeProperty>
  <owl:DatatypeProperty rdf:about="http://example.org/onto/prop/google_data_loss_prevention_deidentify_template_hours">
    <rdfs:label>hours</rdfs:label>
    <rdfs:comment>Hours of day in 24 hour format. Should be from 0 to 23. An API may choose to allow the value "24:00:00" for scenarios like business closing time.</rdfs:comment>
    <rdfs:domain rdf:resource="http://example.org/onto/class/google_data_loss_prevention_deidentify_template"/>
    <rdfs:range rdf:resource="http://www.w3.org/2001/XMLSchema#string"/>
  </owl:DatatypeProperty>
  <owl:DatatypeProperty rdf:about="http://example.org/onto/prop/google_data_loss_prevention_deidentify_template_minutes">
    <rdfs:label>minutes</rdfs:label>
    <rdfs:comment>Minutes of hour of day. Must be from 0 to 59.</rdfs:comment>
    <rdfs:domain rdf:resource="http://example.org/onto/class/google_data_loss_prevention_deidentify_template"/>
    <rdfs:range rdf:resource="http://www.w3.org/2001/XMLSchema#string"/>
  </owl:DatatypeProperty>
  <owl:DatatypeProperty rdf:about="http://example.org/onto/prop/google_data_loss_prevention_deidentify_template_nanos">
    <rdfs:label>nanos</rdfs:label>
    <rdfs:comment>Fractions of seconds in nanoseconds. Must be from 0 to 999,999,999.</rdfs:comment>
    <rdfs:domain rdf:resource="http://example.org/onto/class/google_data_loss_prevention_deidentify_template"/>
    <rdfs:range rdf:resource="http://www.w3.org/2001/XMLSchema#string"/>
  </owl:DatatypeProperty>
  <owl:DatatypeProperty rdf:about="http://example.org/onto/prop/google_data_loss_prevention_deidentify_template_seconds">
    <rdfs:label>seconds</rdfs:label>
    <rdfs:comment>Seconds of minutes of the time. Must normally be from 0 to 59. An API may allow the value 60 if it allows leap-seconds.</rdfs:comment>
    <rdfs:domain rdf:resource="http://example.org/onto/class/google_data_loss_prevention_deidentify_template"/>
    <rdfs:range rdf:resource="http://www.w3.org/2001/XMLSchema#string"/>
  </owl:DatatypeProperty>
  <owl:DatatypeProperty rdf:about="http://example.org/onto/prop/google_data_loss_prevention_deidentify_template_masking_character">
    <rdfs:label>masking_character</rdfs:label>
    <rdfs:comment>Character to use to mask the sensitive values—for example, * for an alphabetic string such as a name, or 0 for a numeric string
such as ZIP code or credit card number. This string must have a length of 1. If not supplied, this value defaults to * for
strings, and 0 for digits.</rdfs:comment>
    <rdfs:domain rdf:resource="http://example.org/onto/class/google_data_loss_prevention_deidentify_template"/>
    <rdfs:range rdf:resource="http://www.w3.org/2001/XMLSchema#string"/>
  </owl:DatatypeProperty>
  <owl:DatatypeProperty rdf:about="http://example.org/onto/prop/google_data_loss_prevention_deidentify_template_number_to_mask">
    <rdfs:label>number_to_mask</rdfs:label>
    <rdfs:comment>Number of characters to mask. If not set, all matching chars will be masked. Skipped characters do not count towards this tally.
If number_to_mask is negative, this denotes inverse masking. Cloud DLP masks all but a number of characters. For example, suppose you have the following values:
- 'masking_character' is *
- 'number_to_mask' is -4
- 'reverse_order' is false
- 'characters_to_ignore' includes -
- Input string is 1234-5678-9012-3456

The resulting de-identified string is ****-****-****-3456. Cloud DLP masks all but the last four characters. If reverseOrder is true, all but the first four characters are masked as 1234-****-****-****.</rdfs:comment>
    <rdfs:domain rdf:resource="http://example.org/onto/class/google_data_loss_prevention_deidentify_template"/>
    <rdfs:range rdf:resource="http://www.w3.org/2001/XMLSchema#string"/>
  </owl:DatatypeProperty>
  <owl:DatatypeProperty rdf:about="http://example.org/onto/prop/google_data_loss_prevention_deidentify_template_reverse_order">
    <rdfs:label>reverse_order</rdfs:label>
    <rdfs:comment>Mask characters in reverse order. For example, if masking_character is 0, number_to_mask is 14, and reverse_order is 'false', then the
input string '1234-5678-9012-3456' is masked as '00000000000000-3456'.</rdfs:comment>
    <rdfs:domain rdf:resource="http://example.org/onto/class/google_data_loss_prevention_deidentify_template"/>
    <rdfs:range rdf:resource="http://www.w3.org/2001/XMLSchema#string"/>
  </owl:DatatypeProperty>
  <owl:DatatypeProperty rdf:about="http://example.org/onto/prop/google_data_loss_prevention_deidentify_template_characters_to_skip">
    <rdfs:label>characters_to_skip</rdfs:label>
    <rdfs:comment>Characters to not transform when masking.</rdfs:comment>
    <rdfs:domain rdf:resource="http://example.org/onto/class/google_data_loss_prevention_deidentify_template"/>
    <rdfs:range rdf:resource="http://www.w3.org/2001/XMLSchema#string"/>
  </owl:DatatypeProperty>
  <owl:DatatypeProperty rdf:about="http://example.org/onto/prop/google_data_loss_prevention_deidentify_template_common_characters_to_ignore">
    <rdfs:label>common_characters_to_ignore</rdfs:label>
    <rdfs:comment>Common characters to not transform when masking. Useful to avoid removing punctuation. Possible values: ["NUMERIC", "ALPHA_UPPER_CASE", "ALPHA_LOWER_CASE", "PUNCTUATION", "WHITESPACE"]</rdfs:comment>
    <rdfs:domain rdf:resource="http://example.org/onto/class/google_data_loss_prevention_deidentify_template"/>
    <rdfs:range rdf:resource="http://www.w3.org/2001/XMLSchema#string"/>
  </owl:DatatypeProperty>
  <owl:DatatypeProperty rdf:about="http://example.org/onto/prop/google_data_loss_prevention_deidentify_template_name">
    <rdfs:label>name</rdfs:label>
    <rdfs:comment>Name describing the field.</rdfs:comment>
    <rdfs:domain rdf:resource="http://example.org/onto/class/google_data_loss_prevention_deidentify_template"/>
    <rdfs:range rdf:resource="http://www.w3.org/2001/XMLSchema#string"/>
  </owl:DatatypeProperty>
  <owl:DatatypeProperty rdf:about="http://example.org/onto/prop/google_data_loss_prevention_deidentify_template_crypto_key_name">
    <rdfs:label>crypto_key_name</rdfs:label>
    <rdfs:comment>The resource name of the KMS CryptoKey to use for unwrapping.</rdfs:comment>
    <rdfs:domain rdf:resource="http://example.org/onto/class/google_data_loss_prevention_deidentify_template"/>
    <rdfs:range rdf:resource="http://www.w3.org/2001/XMLSchema#string"/>
  </owl:DatatypeProperty>
  <owl:DatatypeProperty rdf:about="http://example.org/onto/prop/google_data_loss_prevention_deidentify_template_wrapped_key">
    <rdfs:label>wrapped_key</rdfs:label>
    <rdfs:comment>The wrapped data crypto key.

A base64-encoded string.</rdfs:comment>
    <rdfs:domain rdf:resource="http://example.org/onto/class/google_data_loss_prevention_deidentify_template"/>
    <rdfs:range rdf:resource="http://www.w3.org/2001/XMLSchema#string"/>
  </owl:DatatypeProperty>
  <owl:DatatypeProperty rdf:about="http://example.org/onto/prop/google_data_loss_prevention_deidentify_template_name">
    <rdfs:label>name</rdfs:label>
    <rdfs:comment>Name of the key. This is an arbitrary string used to differentiate different keys. A unique key is generated per name: two separate 'TransientCryptoKey' protos share the same generated key if their names are the same. When the data crypto key is generated, this name is not used in any way (repeating the api call will result in a different key being generated).</rdfs:comment>
    <rdfs:domain rdf:resource="http://example.org/onto/class/google_data_loss_prevention_deidentify_template"/>
    <rdfs:range rdf:resource="http://www.w3.org/2001/XMLSchema#string"/>
  </owl:DatatypeProperty>
  <owl:DatatypeProperty rdf:about="http://example.org/onto/prop/google_data_loss_prevention_deidentify_template_key">
    <rdfs:label>key</rdfs:label>
    <rdfs:comment>A 128/192/256 bit key.

A base64-encoded string.</rdfs:comment>
    <rdfs:domain rdf:resource="http://example.org/onto/class/google_data_loss_prevention_deidentify_template"/>
    <rdfs:range rdf:resource="http://www.w3.org/2001/XMLSchema#string"/>
  </owl:DatatypeProperty>
  <owl:DatatypeProperty rdf:about="http://example.org/onto/prop/google_data_loss_prevention_deidentify_template_name">
    <rdfs:label>name</rdfs:label>
    <rdfs:comment>Name of the information type. Either a name of your choosing when creating a CustomInfoType, or one of the names listed at [https://cloud.google.com/dlp/docs/infotypes-reference](https://cloud.google.com/dlp/docs/infotypes-reference) when specifying a built-in type. When sending Cloud DLP results to Data Catalog, infoType names should conform to the pattern '[A-Za-z0-9$-_]{1,64}'.</rdfs:comment>
    <rdfs:domain rdf:resource="http://example.org/onto/class/google_data_loss_prevention_deidentify_template"/>
    <rdfs:range rdf:resource="http://www.w3.org/2001/XMLSchema#string"/>
  </owl:DatatypeProperty>
  <owl:DatatypeProperty rdf:about="http://example.org/onto/prop/google_data_loss_prevention_deidentify_template_version">
    <rdfs:label>version</rdfs:label>
    <rdfs:comment>Optional version name for this InfoType.</rdfs:comment>
    <rdfs:domain rdf:resource="http://example.org/onto/class/google_data_loss_prevention_deidentify_template"/>
    <rdfs:range rdf:resource="http://www.w3.org/2001/XMLSchema#string"/>
  </owl:DatatypeProperty>
  <owl:DatatypeProperty rdf:about="http://example.org/onto/prop/google_data_loss_prevention_deidentify_template_score">
    <rdfs:label>score</rdfs:label>
    <rdfs:comment>The sensitivity score applied to the resource. Possible values: ["SENSITIVITY_LOW", "SENSITIVITY_MODERATE", "SENSITIVITY_HIGH"]</rdfs:comment>
    <rdfs:domain rdf:resource="http://example.org/onto/class/google_data_loss_prevention_deidentify_template"/>
    <rdfs:range rdf:resource="http://www.w3.org/2001/XMLSchema#string"/>
  </owl:DatatypeProperty>
  <owl:DatatypeProperty rdf:about="http://example.org/onto/prop/google_data_loss_prevention_deidentify_template_crypto_key_name">
    <rdfs:label>crypto_key_name</rdfs:label>
    <rdfs:comment>The resource name of the KMS CryptoKey to use for unwrapping.</rdfs:comment>
    <rdfs:domain rdf:resource="http://example.org/onto/class/google_data_loss_prevention_deidentify_template"/>
    <rdfs:range rdf:resource="http://www.w3.org/2001/XMLSchema#string"/>
  </owl:DatatypeProperty>
  <owl:DatatypeProperty rdf:about="http://example.org/onto/prop/google_data_loss_prevention_deidentify_template_wrapped_key">
    <rdfs:label>wrapped_key</rdfs:label>
    <rdfs:comment>The wrapped data crypto key.

A base64-encoded string.</rdfs:comment>
    <rdfs:domain rdf:resource="http://example.org/onto/class/google_data_loss_prevention_deidentify_template"/>
    <rdfs:range rdf:resource="http://www.w3.org/2001/XMLSchema#string"/>
  </owl:DatatypeProperty>
  <owl:DatatypeProperty rdf:about="http://example.org/onto/prop/google_data_loss_prevention_deidentify_template_name">
    <rdfs:label>name</rdfs:label>
    <rdfs:comment>Name of the key. This is an arbitrary string used to differentiate different keys. A unique key is generated per name: two separate 'TransientCryptoKey' protos share the same generated key if their names are the same. When the data crypto key is generated, this name is not used in any way (repeating the api call will result in a different key being generated).</rdfs:comment>
    <rdfs:domain rdf:resource="http://example.org/onto/class/google_data_loss_prevention_deidentify_template"/>
    <rdfs:range rdf:resource="http://www.w3.org/2001/XMLSchema#string"/>
  </owl:DatatypeProperty>
  <owl:DatatypeProperty rdf:about="http://example.org/onto/prop/google_data_loss_prevention_deidentify_template_key">
    <rdfs:label>key</rdfs:label>
    <rdfs:comment>A 128/192/256 bit key.

A base64-encoded string.</rdfs:comment>
    <rdfs:domain rdf:resource="http://example.org/onto/class/google_data_loss_prevention_deidentify_template"/>
    <rdfs:range rdf:resource="http://www.w3.org/2001/XMLSchema#string"/>
  </owl:DatatypeProperty>
  <owl:DatatypeProperty rdf:about="http://example.org/onto/prop/google_data_loss_prevention_deidentify_template_common_alphabet">
    <rdfs:label>common_alphabet</rdfs:label>
    <rdfs:comment>Common alphabets. Possible values: ["FFX_COMMON_NATIVE_ALPHABET_UNSPECIFIED", "NUMERIC", "HEXADECIMAL", "UPPER_CASE_ALPHA_NUMERIC", "ALPHA_NUMERIC"]</rdfs:comment>
    <rdfs:domain rdf:resource="http://example.org/onto/class/google_data_loss_prevention_deidentify_template"/>
    <rdfs:range rdf:resource="http://www.w3.org/2001/XMLSchema#string"/>
  </owl:DatatypeProperty>
  <owl:DatatypeProperty rdf:about="http://example.org/onto/prop/google_data_loss_prevention_deidentify_template_custom_alphabet">
    <rdfs:label>custom_alphabet</rdfs:label>
    <rdfs:comment>This is supported by mapping these to the alphanumeric characters that the FFX mode natively supports. This happens before/after encryption/decryption. Each character listed must appear only once. Number of characters must be in the range \[2, 95\]. This must be encoded as ASCII. The order of characters does not matter. The full list of allowed characters is:

''0123456789ABCDEFGHIJKLMNOPQRSTUVWXYZabcdefghijklmnopqrstuvwxyz ~'!@#$%^&*()_-+={[}]|:;"'<,>.?/''</rdfs:comment>
    <rdfs:domain rdf:resource="http://example.org/onto/class/google_data_loss_prevention_deidentify_template"/>
    <rdfs:range rdf:resource="http://www.w3.org/2001/XMLSchema#string"/>
  </owl:DatatypeProperty>
  <owl:DatatypeProperty rdf:about="http://example.org/onto/prop/google_data_loss_prevention_deidentify_template_radix">
    <rdfs:label>radix</rdfs:label>
    <rdfs:comment>The native way to select the alphabet. Must be in the range \[2, 95\].</rdfs:comment>
    <rdfs:domain rdf:resource="http://example.org/onto/class/google_data_loss_prevention_deidentify_template"/>
    <rdfs:range rdf:resource="http://www.w3.org/2001/XMLSchema#string"/>
  </owl:DatatypeProperty>
  <owl:DatatypeProperty rdf:about="http://example.org/onto/prop/google_data_loss_prevention_deidentify_template_name">
    <rdfs:label>name</rdfs:label>
    <rdfs:comment>Name describing the field.</rdfs:comment>
    <rdfs:domain rdf:resource="http://example.org/onto/class/google_data_loss_prevention_deidentify_template"/>
    <rdfs:range rdf:resource="http://www.w3.org/2001/XMLSchema#string"/>
  </owl:DatatypeProperty>
  <owl:DatatypeProperty rdf:about="http://example.org/onto/prop/google_data_loss_prevention_deidentify_template_crypto_key_name">
    <rdfs:label>crypto_key_name</rdfs:label>
    <rdfs:comment>The resource name of the KMS CryptoKey to use for unwrapping.</rdfs:comment>
    <rdfs:domain rdf:resource="http://example.org/onto/class/google_data_loss_prevention_deidentify_template"/>
    <rdfs:range rdf:resource="http://www.w3.org/2001/XMLSchema#string"/>
  </owl:DatatypeProperty>
  <owl:DatatypeProperty rdf:about="http://example.org/onto/prop/google_data_loss_prevention_deidentify_template_wrapped_key">
    <rdfs:label>wrapped_key</rdfs:label>
    <rdfs:comment>The wrapped data crypto key.

A base64-encoded string.</rdfs:comment>
    <rdfs:domain rdf:resource="http://example.org/onto/class/google_data_loss_prevention_deidentify_template"/>
    <rdfs:range rdf:resource="http://www.w3.org/2001/XMLSchema#string"/>
  </owl:DatatypeProperty>
  <owl:DatatypeProperty rdf:about="http://example.org/onto/prop/google_data_loss_prevention_deidentify_template_name">
    <rdfs:label>name</rdfs:label>
    <rdfs:comment>Name of the key. This is an arbitrary string used to differentiate different keys. A unique key is generated per name: two separate 'TransientCryptoKey' protos share the same generated key if their names are the same. When the data crypto key is generated, this name is not used in any way (repeating the api call will result in a different key being generated).</rdfs:comment>
    <rdfs:domain rdf:resource="http://example.org/onto/class/google_data_loss_prevention_deidentify_template"/>
    <rdfs:range rdf:resource="http://www.w3.org/2001/XMLSchema#string"/>
  </owl:DatatypeProperty>
  <owl:DatatypeProperty rdf:about="http://example.org/onto/prop/google_data_loss_prevention_deidentify_template_key">
    <rdfs:label>key</rdfs:label>
    <rdfs:comment>A 128/192/256 bit key.

A base64-encoded string.</rdfs:comment>
    <rdfs:domain rdf:resource="http://example.org/onto/class/google_data_loss_prevention_deidentify_template"/>
    <rdfs:range rdf:resource="http://www.w3.org/2001/XMLSchema#string"/>
  </owl:DatatypeProperty>
  <owl:DatatypeProperty rdf:about="http://example.org/onto/prop/google_data_loss_prevention_deidentify_template_name">
    <rdfs:label>name</rdfs:label>
    <rdfs:comment>Name of the information type. Either a name of your choosing when creating a CustomInfoType, or one of the names listed at [https://cloud.google.com/dlp/docs/infotypes-reference](https://cloud.google.com/dlp/docs/infotypes-reference) when specifying a built-in type. When sending Cloud DLP results to Data Catalog, infoType names should conform to the pattern '[A-Za-z0-9$-_]{1,64}'.</rdfs:comment>
    <rdfs:domain rdf:resource="http://example.org/onto/class/google_data_loss_prevention_deidentify_template"/>
    <rdfs:range rdf:resource="http://www.w3.org/2001/XMLSchema#string"/>
  </owl:DatatypeProperty>
  <owl:DatatypeProperty rdf:about="http://example.org/onto/prop/google_data_loss_prevention_deidentify_template_version">
    <rdfs:label>version</rdfs:label>
    <rdfs:comment>Optional version name for this InfoType.</rdfs:comment>
    <rdfs:domain rdf:resource="http://example.org/onto/class/google_data_loss_prevention_deidentify_template"/>
    <rdfs:range rdf:resource="http://www.w3.org/2001/XMLSchema#string"/>
  </owl:DatatypeProperty>
  <owl:DatatypeProperty rdf:about="http://example.org/onto/prop/google_data_loss_prevention_deidentify_template_score">
    <rdfs:label>score</rdfs:label>
    <rdfs:comment>The sensitivity score applied to the resource. Possible values: ["SENSITIVITY_LOW", "SENSITIVITY_MODERATE", "SENSITIVITY_HIGH"]</rdfs:comment>
    <rdfs:domain rdf:resource="http://example.org/onto/class/google_data_loss_prevention_deidentify_template"/>
    <rdfs:range rdf:resource="http://www.w3.org/2001/XMLSchema#string"/>
  </owl:DatatypeProperty>
  <owl:DatatypeProperty rdf:about="http://example.org/onto/prop/google_data_loss_prevention_deidentify_template_lower_bound_days">
    <rdfs:label>lower_bound_days</rdfs:label>
    <rdfs:comment>For example, -5 means shift date to at most 5 days back in the past.</rdfs:comment>
    <rdfs:domain rdf:resource="http://example.org/onto/class/google_data_loss_prevention_deidentify_template"/>
    <rdfs:range rdf:resource="http://www.w3.org/2001/XMLSchema#string"/>
  </owl:DatatypeProperty>
  <owl:DatatypeProperty rdf:about="http://example.org/onto/prop/google_data_loss_prevention_deidentify_template_upper_bound_days">
    <rdfs:label>upper_bound_days</rdfs:label>
    <rdfs:comment>Range of shift in days. Actual shift will be selected at random within this range (inclusive ends). Negative means shift to earlier in time. Must not be more than 365250 days (1000 years) each direction.

For example, 3 means shift date to at most 3 days into the future.</rdfs:comment>
    <rdfs:domain rdf:resource="http://example.org/onto/class/google_data_loss_prevention_deidentify_template"/>
    <rdfs:range rdf:resource="http://www.w3.org/2001/XMLSchema#string"/>
  </owl:DatatypeProperty>
  <owl:DatatypeProperty rdf:about="http://example.org/onto/prop/google_data_loss_prevention_deidentify_template_name">
    <rdfs:label>name</rdfs:label>
    <rdfs:comment>Name describing the field.</rdfs:comment>
    <rdfs:domain rdf:resource="http://example.org/onto/class/google_data_loss_prevention_deidentify_template"/>
    <rdfs:range rdf:resource="http://www.w3.org/2001/XMLSchema#string"/>
  </owl:DatatypeProperty>
  <owl:DatatypeProperty rdf:about="http://example.org/onto/prop/google_data_loss_prevention_deidentify_template_crypto_key_name">
    <rdfs:label>crypto_key_name</rdfs:label>
    <rdfs:comment>The resource name of the KMS CryptoKey to use for unwrapping.</rdfs:comment>
    <rdfs:domain rdf:resource="http://example.org/onto/class/google_data_loss_prevention_deidentify_template"/>
    <rdfs:range rdf:resource="http://www.w3.org/2001/XMLSchema#string"/>
  </owl:DatatypeProperty>
  <owl:DatatypeProperty rdf:about="http://example.org/onto/prop/google_data_loss_prevention_deidentify_template_wrapped_key">
    <rdfs:label>wrapped_key</rdfs:label>
    <rdfs:comment>The wrapped data crypto key.

A base64-encoded string.</rdfs:comment>
    <rdfs:domain rdf:resource="http://example.org/onto/class/google_data_loss_prevention_deidentify_template"/>
    <rdfs:range rdf:resource="http://www.w3.org/2001/XMLSchema#string"/>
  </owl:DatatypeProperty>
  <owl:DatatypeProperty rdf:about="http://example.org/onto/prop/google_data_loss_prevention_deidentify_template_name">
    <rdfs:label>name</rdfs:label>
    <rdfs:comment>Name of the key. This is an arbitrary string used to differentiate different keys. A unique key is generated per name: two separate 'TransientCryptoKey' protos share the same generated key if their names are the same. When the data crypto key is generated, this name is not used in any way (repeating the api call will result in a different key being generated).</rdfs:comment>
    <rdfs:domain rdf:resource="http://example.org/onto/class/google_data_loss_prevention_deidentify_template"/>
    <rdfs:range rdf:resource="http://www.w3.org/2001/XMLSchema#string"/>
  </owl:DatatypeProperty>
  <owl:DatatypeProperty rdf:about="http://example.org/onto/prop/google_data_loss_prevention_deidentify_template_key">
    <rdfs:label>key</rdfs:label>
    <rdfs:comment>A 128/192/256 bit key.

A base64-encoded string.</rdfs:comment>
    <rdfs:domain rdf:resource="http://example.org/onto/class/google_data_loss_prevention_deidentify_template"/>
    <rdfs:range rdf:resource="http://www.w3.org/2001/XMLSchema#string"/>
  </owl:DatatypeProperty>
  <owl:DatatypeProperty rdf:about="http://example.org/onto/prop/google_data_loss_prevention_deidentify_template_bucket_size">
    <rdfs:label>bucket_size</rdfs:label>
    <rdfs:comment>Size of each bucket (except for minimum and maximum buckets).
So if lower_bound = 10, upper_bound = 89, and bucketSize = 10, then the following buckets would be used: -10, 10-20, 20-30, 30-40, 40-50, 50-60, 60-70, 70-80, 80-89, 89+.
Precision up to 2 decimals works.</rdfs:comment>
    <rdfs:domain rdf:resource="http://example.org/onto/class/google_data_loss_prevention_deidentify_template"/>
    <rdfs:range rdf:resource="http://www.w3.org/2001/XMLSchema#string"/>
  </owl:DatatypeProperty>
  <owl:DatatypeProperty rdf:about="http://example.org/onto/prop/google_data_loss_prevention_deidentify_template_boolean_value">
    <rdfs:label>boolean_value</rdfs:label>
    <rdfs:comment>A boolean value.</rdfs:comment>
    <rdfs:domain rdf:resource="http://example.org/onto/class/google_data_loss_prevention_deidentify_template"/>
    <rdfs:range rdf:resource="http://www.w3.org/2001/XMLSchema#string"/>
  </owl:DatatypeProperty>
  <owl:DatatypeProperty rdf:about="http://example.org/onto/prop/google_data_loss_prevention_deidentify_template_day_of_week_value">
    <rdfs:label>day_of_week_value</rdfs:label>
    <rdfs:comment>Represents a day of the week. Possible values: ["MONDAY", "TUESDAY", "WEDNESDAY", "THURSDAY", "FRIDAY", "SATURDAY", "SUNDAY"]</rdfs:comment>
    <rdfs:domain rdf:resource="http://example.org/onto/class/google_data_loss_prevention_deidentify_template"/>
    <rdfs:range rdf:resource="http://www.w3.org/2001/XMLSchema#string"/>
  </owl:DatatypeProperty>
  <owl:DatatypeProperty rdf:about="http://example.org/onto/prop/google_data_loss_prevention_deidentify_template_float_value">
    <rdfs:label>float_value</rdfs:label>
    <rdfs:comment>A float value.</rdfs:comment>
    <rdfs:domain rdf:resource="http://example.org/onto/class/google_data_loss_prevention_deidentify_template"/>
    <rdfs:range rdf:resource="http://www.w3.org/2001/XMLSchema#string"/>
  </owl:DatatypeProperty>
  <owl:DatatypeProperty rdf:about="http://example.org/onto/prop/google_data_loss_prevention_deidentify_template_integer_value">
    <rdfs:label>integer_value</rdfs:label>
    <rdfs:comment>An integer value (int64 format)</rdfs:comment>
    <rdfs:domain rdf:resource="http://example.org/onto/class/google_data_loss_prevention_deidentify_template"/>
    <rdfs:range rdf:resource="http://www.w3.org/2001/XMLSchema#string"/>
  </owl:DatatypeProperty>
  <owl:DatatypeProperty rdf:about="http://example.org/onto/prop/google_data_loss_prevention_deidentify_template_string_value">
    <rdfs:label>string_value</rdfs:label>
    <rdfs:comment>A string value.</rdfs:comment>
    <rdfs:domain rdf:resource="http://example.org/onto/class/google_data_loss_prevention_deidentify_template"/>
    <rdfs:range rdf:resource="http://www.w3.org/2001/XMLSchema#string"/>
  </owl:DatatypeProperty>
  <owl:DatatypeProperty rdf:about="http://example.org/onto/prop/google_data_loss_prevention_deidentify_template_timestamp_value">
    <rdfs:label>timestamp_value</rdfs:label>
    <rdfs:comment>A timestamp in RFC3339 UTC "Zulu" format, with nanosecond resolution and up to nine fractional digits. Examples: "2014-10-02T15:01:23Z" and "2014-10-02T15:01:23.045123456Z".</rdfs:comment>
    <rdfs:domain rdf:resource="http://example.org/onto/class/google_data_loss_prevention_deidentify_template"/>
    <rdfs:range rdf:resource="http://www.w3.org/2001/XMLSchema#string"/>
  </owl:DatatypeProperty>
  <owl:DatatypeProperty rdf:about="http://example.org/onto/prop/google_data_loss_prevention_deidentify_template_day">
    <rdfs:label>day</rdfs:label>
    <rdfs:comment>Day of a month. Must be from 1 to 31 and valid for the year and month, or 0 to specify a year by itself or a year and month where the day isn't significant.</rdfs:comment>
    <rdfs:domain rdf:resource="http://example.org/onto/class/google_data_loss_prevention_deidentify_template"/>
    <rdfs:range rdf:resource="http://www.w3.org/2001/XMLSchema#string"/>
  </owl:DatatypeProperty>
  <owl:DatatypeProperty rdf:about="http://example.org/onto/prop/google_data_loss_prevention_deidentify_template_month">
    <rdfs:label>month</rdfs:label>
    <rdfs:comment>Month of a year. Must be from 1 to 12, or 0 to specify a year without a month and day.</rdfs:comment>
    <rdfs:domain rdf:resource="http://example.org/onto/class/google_data_loss_prevention_deidentify_template"/>
    <rdfs:range rdf:resource="http://www.w3.org/2001/XMLSchema#string"/>
  </owl:DatatypeProperty>
  <owl:DatatypeProperty rdf:about="http://example.org/onto/prop/google_data_loss_prevention_deidentify_template_year">
    <rdfs:label>year</rdfs:label>
    <rdfs:comment>Year of the date. Must be from 1 to 9999, or 0 to specify a date without a year.</rdfs:comment>
    <rdfs:domain rdf:resource="http://example.org/onto/class/google_data_loss_prevention_deidentify_template"/>
    <rdfs:range rdf:resource="http://www.w3.org/2001/XMLSchema#string"/>
  </owl:DatatypeProperty>
  <owl:DatatypeProperty rdf:about="http://example.org/onto/prop/google_data_loss_prevention_deidentify_template_hours">
    <rdfs:label>hours</rdfs:label>
    <rdfs:comment>Hours of day in 24 hour format. Should be from 0 to 23. An API may choose to allow the value "24:00:00" for scenarios like business closing time.</rdfs:comment>
    <rdfs:domain rdf:resource="http://example.org/onto/class/google_data_loss_prevention_deidentify_template"/>
    <rdfs:range rdf:resource="http://www.w3.org/2001/XMLSchema#string"/>
  </owl:DatatypeProperty>
  <owl:DatatypeProperty rdf:about="http://example.org/onto/prop/google_data_loss_prevention_deidentify_template_minutes">
    <rdfs:label>minutes</rdfs:label>
    <rdfs:comment>Minutes of hour of day. Must be from 0 to 59.</rdfs:comment>
    <rdfs:domain rdf:resource="http://example.org/onto/class/google_data_loss_prevention_deidentify_template"/>
    <rdfs:range rdf:resource="http://www.w3.org/2001/XMLSchema#string"/>
  </owl:DatatypeProperty>
  <owl:DatatypeProperty rdf:about="http://example.org/onto/prop/google_data_loss_prevention_deidentify_template_nanos">
    <rdfs:label>nanos</rdfs:label>
    <rdfs:comment>Fractions of seconds in nanoseconds. Must be from 0 to 999,999,999.</rdfs:comment>
    <rdfs:domain rdf:resource="http://example.org/onto/class/google_data_loss_prevention_deidentify_template"/>
    <rdfs:range rdf:resource="http://www.w3.org/2001/XMLSchema#string"/>
  </owl:DatatypeProperty>
  <owl:DatatypeProperty rdf:about="http://example.org/onto/prop/google_data_loss_prevention_deidentify_template_seconds">
    <rdfs:label>seconds</rdfs:label>
    <rdfs:comment>Seconds of minutes of the time. Must normally be from 0 to 59. An API may allow the value 60 if it allows leap-seconds.</rdfs:comment>
    <rdfs:domain rdf:resource="http://example.org/onto/class/google_data_loss_prevention_deidentify_template"/>
    <rdfs:range rdf:resource="http://www.w3.org/2001/XMLSchema#string"/>
  </owl:DatatypeProperty>
  <owl:DatatypeProperty rdf:about="http://example.org/onto/prop/google_data_loss_prevention_deidentify_template_boolean_value">
    <rdfs:label>boolean_value</rdfs:label>
    <rdfs:comment>A boolean value.</rdfs:comment>
    <rdfs:domain rdf:resource="http://example.org/onto/class/google_data_loss_prevention_deidentify_template"/>
    <rdfs:range rdf:resource="http://www.w3.org/2001/XMLSchema#string"/>
  </owl:DatatypeProperty>
  <owl:DatatypeProperty rdf:about="http://example.org/onto/prop/google_data_loss_prevention_deidentify_template_day_of_week_value">
    <rdfs:label>day_of_week_value</rdfs:label>
    <rdfs:comment>Represents a day of the week. Possible values: ["MONDAY", "TUESDAY", "WEDNESDAY", "THURSDAY", "FRIDAY", "SATURDAY", "SUNDAY"]</rdfs:comment>
    <rdfs:domain rdf:resource="http://example.org/onto/class/google_data_loss_prevention_deidentify_template"/>
    <rdfs:range rdf:resource="http://www.w3.org/2001/XMLSchema#string"/>
  </owl:DatatypeProperty>
  <owl:DatatypeProperty rdf:about="http://example.org/onto/prop/google_data_loss_prevention_deidentify_template_float_value">
    <rdfs:label>float_value</rdfs:label>
    <rdfs:comment>A float value.</rdfs:comment>
    <rdfs:domain rdf:resource="http://example.org/onto/class/google_data_loss_prevention_deidentify_template"/>
    <rdfs:range rdf:resource="http://www.w3.org/2001/XMLSchema#string"/>
  </owl:DatatypeProperty>
  <owl:DatatypeProperty rdf:about="http://example.org/onto/prop/google_data_loss_prevention_deidentify_template_integer_value">
    <rdfs:label>integer_value</rdfs:label>
    <rdfs:comment>An integer value (int64 format)</rdfs:comment>
    <rdfs:domain rdf:resource="http://example.org/onto/class/google_data_loss_prevention_deidentify_template"/>
    <rdfs:range rdf:resource="http://www.w3.org/2001/XMLSchema#string"/>
  </owl:DatatypeProperty>
  <owl:DatatypeProperty rdf:about="http://example.org/onto/prop/google_data_loss_prevention_deidentify_template_string_value">
    <rdfs:label>string_value</rdfs:label>
    <rdfs:comment>A string value.</rdfs:comment>
    <rdfs:domain rdf:resource="http://example.org/onto/class/google_data_loss_prevention_deidentify_template"/>
    <rdfs:range rdf:resource="http://www.w3.org/2001/XMLSchema#string"/>
  </owl:DatatypeProperty>
  <owl:DatatypeProperty rdf:about="http://example.org/onto/prop/google_data_loss_prevention_deidentify_template_timestamp_value">
    <rdfs:label>timestamp_value</rdfs:label>
    <rdfs:comment>A timestamp in RFC3339 UTC "Zulu" format, with nanosecond resolution and up to nine fractional digits. Examples: "2014-10-02T15:01:23Z" and "2014-10-02T15:01:23.045123456Z".</rdfs:comment>
    <rdfs:domain rdf:resource="http://example.org/onto/class/google_data_loss_prevention_deidentify_template"/>
    <rdfs:range rdf:resource="http://www.w3.org/2001/XMLSchema#string"/>
  </owl:DatatypeProperty>
  <owl:DatatypeProperty rdf:about="http://example.org/onto/prop/google_data_loss_prevention_deidentify_template_day">
    <rdfs:label>day</rdfs:label>
    <rdfs:comment>Day of a month. Must be from 1 to 31 and valid for the year and month, or 0 to specify a year by itself or a year and month where the day isn't significant.</rdfs:comment>
    <rdfs:domain rdf:resource="http://example.org/onto/class/google_data_loss_prevention_deidentify_template"/>
    <rdfs:range rdf:resource="http://www.w3.org/2001/XMLSchema#string"/>
  </owl:DatatypeProperty>
  <owl:DatatypeProperty rdf:about="http://example.org/onto/prop/google_data_loss_prevention_deidentify_template_month">
    <rdfs:label>month</rdfs:label>
    <rdfs:comment>Month of a year. Must be from 1 to 12, or 0 to specify a year without a month and day.</rdfs:comment>
    <rdfs:domain rdf:resource="http://example.org/onto/class/google_data_loss_prevention_deidentify_template"/>
    <rdfs:range rdf:resource="http://www.w3.org/2001/XMLSchema#string"/>
  </owl:DatatypeProperty>
  <owl:DatatypeProperty rdf:about="http://example.org/onto/prop/google_data_loss_prevention_deidentify_template_year">
    <rdfs:label>year</rdfs:label>
    <rdfs:comment>Year of the date. Must be from 1 to 9999, or 0 to specify a date without a year.</rdfs:comment>
    <rdfs:domain rdf:resource="http://example.org/onto/class/google_data_loss_prevention_deidentify_template"/>
    <rdfs:range rdf:resource="http://www.w3.org/2001/XMLSchema#string"/>
  </owl:DatatypeProperty>
  <owl:DatatypeProperty rdf:about="http://example.org/onto/prop/google_data_loss_prevention_deidentify_template_hours">
    <rdfs:label>hours</rdfs:label>
    <rdfs:comment>Hours of day in 24 hour format. Should be from 0 to 23. An API may choose to allow the value "24:00:00" for scenarios like business closing time.</rdfs:comment>
    <rdfs:domain rdf:resource="http://example.org/onto/class/google_data_loss_prevention_deidentify_template"/>
    <rdfs:range rdf:resource="http://www.w3.org/2001/XMLSchema#string"/>
  </owl:DatatypeProperty>
  <owl:DatatypeProperty rdf:about="http://example.org/onto/prop/google_data_loss_prevention_deidentify_template_minutes">
    <rdfs:label>minutes</rdfs:label>
    <rdfs:comment>Minutes of hour of day. Must be from 0 to 59.</rdfs:comment>
    <rdfs:domain rdf:resource="http://example.org/onto/class/google_data_loss_prevention_deidentify_template"/>
    <rdfs:range rdf:resource="http://www.w3.org/2001/XMLSchema#string"/>
  </owl:DatatypeProperty>
  <owl:DatatypeProperty rdf:about="http://example.org/onto/prop/google_data_loss_prevention_deidentify_template_nanos">
    <rdfs:label>nanos</rdfs:label>
    <rdfs:comment>Fractions of seconds in nanoseconds. Must be from 0 to 999,999,999.</rdfs:comment>
    <rdfs:domain rdf:resource="http://example.org/onto/class/google_data_loss_prevention_deidentify_template"/>
    <rdfs:range rdf:resource="http://www.w3.org/2001/XMLSchema#string"/>
  </owl:DatatypeProperty>
  <owl:DatatypeProperty rdf:about="http://example.org/onto/prop/google_data_loss_prevention_deidentify_template_seconds">
    <rdfs:label>seconds</rdfs:label>
    <rdfs:comment>Seconds of minutes of the time. Must normally be from 0 to 59. An API may allow the value 60 if it allows leap-seconds.</rdfs:comment>
    <rdfs:domain rdf:resource="http://example.org/onto/class/google_data_loss_prevention_deidentify_template"/>
    <rdfs:range rdf:resource="http://www.w3.org/2001/XMLSchema#string"/>
  </owl:DatatypeProperty>
  <owl:DatatypeProperty rdf:about="http://example.org/onto/prop/google_data_loss_prevention_deidentify_template_boolean_value">
    <rdfs:label>boolean_value</rdfs:label>
    <rdfs:comment>A boolean value.</rdfs:comment>
    <rdfs:domain rdf:resource="http://example.org/onto/class/google_data_loss_prevention_deidentify_template"/>
    <rdfs:range rdf:resource="http://www.w3.org/2001/XMLSchema#string"/>
  </owl:DatatypeProperty>
  <owl:DatatypeProperty rdf:about="http://example.org/onto/prop/google_data_loss_prevention_deidentify_template_day_of_week_value">
    <rdfs:label>day_of_week_value</rdfs:label>
    <rdfs:comment>Represents a day of the week. Possible values: ["MONDAY", "TUESDAY", "WEDNESDAY", "THURSDAY", "FRIDAY", "SATURDAY", "SUNDAY"]</rdfs:comment>
    <rdfs:domain rdf:resource="http://example.org/onto/class/google_data_loss_prevention_deidentify_template"/>
    <rdfs:range rdf:resource="http://www.w3.org/2001/XMLSchema#string"/>
  </owl:DatatypeProperty>
  <owl:DatatypeProperty rdf:about="http://example.org/onto/prop/google_data_loss_prevention_deidentify_template_float_value">
    <rdfs:label>float_value</rdfs:label>
    <rdfs:comment>A float value.</rdfs:comment>
    <rdfs:domain rdf:resource="http://example.org/onto/class/google_data_loss_prevention_deidentify_template"/>
    <rdfs:range rdf:resource="http://www.w3.org/2001/XMLSchema#string"/>
  </owl:DatatypeProperty>
  <owl:DatatypeProperty rdf:about="http://example.org/onto/prop/google_data_loss_prevention_deidentify_template_integer_value">
    <rdfs:label>integer_value</rdfs:label>
    <rdfs:comment>An integer value (int64 format)</rdfs:comment>
    <rdfs:domain rdf:resource="http://example.org/onto/class/google_data_loss_prevention_deidentify_template"/>
    <rdfs:range rdf:resource="http://www.w3.org/2001/XMLSchema#string"/>
  </owl:DatatypeProperty>
  <owl:DatatypeProperty rdf:about="http://example.org/onto/prop/google_data_loss_prevention_deidentify_template_string_value">
    <rdfs:label>string_value</rdfs:label>
    <rdfs:comment>A string value.</rdfs:comment>
    <rdfs:domain rdf:resource="http://example.org/onto/class/google_data_loss_prevention_deidentify_template"/>
    <rdfs:range rdf:resource="http://www.w3.org/2001/XMLSchema#string"/>
  </owl:DatatypeProperty>
  <owl:DatatypeProperty rdf:about="http://example.org/onto/prop/google_data_loss_prevention_deidentify_template_timestamp_value">
    <rdfs:label>timestamp_value</rdfs:label>
    <rdfs:comment>A timestamp in RFC3339 UTC "Zulu" format, with nanosecond resolution and up to nine fractional digits. Examples: "2014-10-02T15:01:23Z" and "2014-10-02T15:01:23.045123456Z".</rdfs:comment>
    <rdfs:domain rdf:resource="http://example.org/onto/class/google_data_loss_prevention_deidentify_template"/>
    <rdfs:range rdf:resource="http://www.w3.org/2001/XMLSchema#string"/>
  </owl:DatatypeProperty>
  <owl:DatatypeProperty rdf:about="http://example.org/onto/prop/google_data_loss_prevention_deidentify_template_day">
    <rdfs:label>day</rdfs:label>
    <rdfs:comment>Day of a month. Must be from 1 to 31 and valid for the year and month, or 0 to specify a year by itself or a year and month where the day isn't significant.</rdfs:comment>
    <rdfs:domain rdf:resource="http://example.org/onto/class/google_data_loss_prevention_deidentify_template"/>
    <rdfs:range rdf:resource="http://www.w3.org/2001/XMLSchema#string"/>
  </owl:DatatypeProperty>
  <owl:DatatypeProperty rdf:about="http://example.org/onto/prop/google_data_loss_prevention_deidentify_template_month">
    <rdfs:label>month</rdfs:label>
    <rdfs:comment>Month of a year. Must be from 1 to 12, or 0 to specify a year without a month and day.</rdfs:comment>
    <rdfs:domain rdf:resource="http://example.org/onto/class/google_data_loss_prevention_deidentify_template"/>
    <rdfs:range rdf:resource="http://www.w3.org/2001/XMLSchema#string"/>
  </owl:DatatypeProperty>
  <owl:DatatypeProperty rdf:about="http://example.org/onto/prop/google_data_loss_prevention_deidentify_template_year">
    <rdfs:label>year</rdfs:label>
    <rdfs:comment>Year of the date. Must be from 1 to 9999, or 0 to specify a date without a year.</rdfs:comment>
    <rdfs:domain rdf:resource="http://example.org/onto/class/google_data_loss_prevention_deidentify_template"/>
    <rdfs:range rdf:resource="http://www.w3.org/2001/XMLSchema#string"/>
  </owl:DatatypeProperty>
  <owl:DatatypeProperty rdf:about="http://example.org/onto/prop/google_data_loss_prevention_deidentify_template_hours">
    <rdfs:label>hours</rdfs:label>
    <rdfs:comment>Hours of day in 24 hour format. Should be from 0 to 23. An API may choose to allow the value "24:00:00" for scenarios like business closing time.</rdfs:comment>
    <rdfs:domain rdf:resource="http://example.org/onto/class/google_data_loss_prevention_deidentify_template"/>
    <rdfs:range rdf:resource="http://www.w3.org/2001/XMLSchema#string"/>
  </owl:DatatypeProperty>
  <owl:DatatypeProperty rdf:about="http://example.org/onto/prop/google_data_loss_prevention_deidentify_template_minutes">
    <rdfs:label>minutes</rdfs:label>
    <rdfs:comment>Minutes of hour of day. Must be from 0 to 59.</rdfs:comment>
    <rdfs:domain rdf:resource="http://example.org/onto/class/google_data_loss_prevention_deidentify_template"/>
    <rdfs:range rdf:resource="http://www.w3.org/2001/XMLSchema#string"/>
  </owl:DatatypeProperty>
  <owl:DatatypeProperty rdf:about="http://example.org/onto/prop/google_data_loss_prevention_deidentify_template_nanos">
    <rdfs:label>nanos</rdfs:label>
    <rdfs:comment>Fractions of seconds in nanoseconds. Must be from 0 to 999,999,999.</rdfs:comment>
    <rdfs:domain rdf:resource="http://example.org/onto/class/google_data_loss_prevention_deidentify_template"/>
    <rdfs:range rdf:resource="http://www.w3.org/2001/XMLSchema#string"/>
  </owl:DatatypeProperty>
  <owl:DatatypeProperty rdf:about="http://example.org/onto/prop/google_data_loss_prevention_deidentify_template_seconds">
    <rdfs:label>seconds</rdfs:label>
    <rdfs:comment>Seconds of minutes of the time. Must normally be from 0 to 59. An API may allow the value 60 if it allows leap-seconds.</rdfs:comment>
    <rdfs:domain rdf:resource="http://example.org/onto/class/google_data_loss_prevention_deidentify_template"/>
    <rdfs:range rdf:resource="http://www.w3.org/2001/XMLSchema#string"/>
  </owl:DatatypeProperty>
  <owl:DatatypeProperty rdf:about="http://example.org/onto/prop/google_data_loss_prevention_deidentify_template_words">
    <rdfs:label>words</rdfs:label>
    <rdfs:comment>Words or phrases defining the dictionary. The dictionary must contain at least one phrase and every phrase must contain at least 2 characters that are letters or digits.</rdfs:comment>
    <rdfs:domain rdf:resource="http://example.org/onto/class/google_data_loss_prevention_deidentify_template"/>
    <rdfs:range rdf:resource="http://www.w3.org/2001/XMLSchema#string"/>
  </owl:DatatypeProperty>
  <owl:DatatypeProperty rdf:about="http://example.org/onto/prop/google_data_loss_prevention_deidentify_template_part_to_extract">
    <rdfs:label>part_to_extract</rdfs:label>
    <rdfs:comment>The part of the time to keep. Possible values: ["YEAR", "MONTH", "DAY_OF_MONTH", "DAY_OF_WEEK", "WEEK_OF_YEAR", "HOUR_OF_DAY"]</rdfs:comment>
    <rdfs:domain rdf:resource="http://example.org/onto/class/google_data_loss_prevention_deidentify_template"/>
    <rdfs:range rdf:resource="http://www.w3.org/2001/XMLSchema#string"/>
  </owl:DatatypeProperty>
  <owl:DatatypeProperty rdf:about="http://example.org/onto/prop/google_data_loss_prevention_deidentify_template_logical_operator">
    <rdfs:label>logical_operator</rdfs:label>
    <rdfs:comment>The operator to apply to the result of conditions. Default and currently only supported value is AND. Default value: "AND" Possible values: ["AND"]</rdfs:comment>
    <rdfs:domain rdf:resource="http://example.org/onto/class/google_data_loss_prevention_deidentify_template"/>
    <rdfs:range rdf:resource="http://www.w3.org/2001/XMLSchema#string"/>
  </owl:DatatypeProperty>
  <owl:DatatypeProperty rdf:about="http://example.org/onto/prop/google_data_loss_prevention_deidentify_template_operator">
    <rdfs:label>operator</rdfs:label>
    <rdfs:comment>Operator used to compare the field or infoType to the value. Possible values: ["EQUAL_TO", "NOT_EQUAL_TO", "GREATER_THAN", "LESS_THAN", "GREATER_THAN_OR_EQUALS", "LESS_THAN_OR_EQUALS", "EXISTS"]</rdfs:comment>
    <rdfs:domain rdf:resource="http://example.org/onto/class/google_data_loss_prevention_deidentify_template"/>
    <rdfs:range rdf:resource="http://www.w3.org/2001/XMLSchema#string"/>
  </owl:DatatypeProperty>
  <owl:DatatypeProperty rdf:about="http://example.org/onto/prop/google_data_loss_prevention_deidentify_template_name">
    <rdfs:label>name</rdfs:label>
    <rdfs:comment>Name describing the field.</rdfs:comment>
    <rdfs:domain rdf:resource="http://example.org/onto/class/google_data_loss_prevention_deidentify_template"/>
    <rdfs:range rdf:resource="http://www.w3.org/2001/XMLSchema#string"/>
  </owl:DatatypeProperty>
  <owl:DatatypeProperty rdf:about="http://example.org/onto/prop/google_data_loss_prevention_deidentify_template_boolean_value">
    <rdfs:label>boolean_value</rdfs:label>
    <rdfs:comment>A boolean value.</rdfs:comment>
    <rdfs:domain rdf:resource="http://example.org/onto/class/google_data_loss_prevention_deidentify_template"/>
    <rdfs:range rdf:resource="http://www.w3.org/2001/XMLSchema#string"/>
  </owl:DatatypeProperty>
  <owl:DatatypeProperty rdf:about="http://example.org/onto/prop/google_data_loss_prevention_deidentify_template_day_of_week_value">
    <rdfs:label>day_of_week_value</rdfs:label>
    <rdfs:comment>Represents a day of the week. Possible values: ["MONDAY", "TUESDAY", "WEDNESDAY", "THURSDAY", "FRIDAY", "SATURDAY", "SUNDAY"]</rdfs:comment>
    <rdfs:domain rdf:resource="http://example.org/onto/class/google_data_loss_prevention_deidentify_template"/>
    <rdfs:range rdf:resource="http://www.w3.org/2001/XMLSchema#string"/>
  </owl:DatatypeProperty>
  <owl:DatatypeProperty rdf:about="http://example.org/onto/prop/google_data_loss_prevention_deidentify_template_float_value">
    <rdfs:label>float_value</rdfs:label>
    <rdfs:comment>A float value.</rdfs:comment>
    <rdfs:domain rdf:resource="http://example.org/onto/class/google_data_loss_prevention_deidentify_template"/>
    <rdfs:range rdf:resource="http://www.w3.org/2001/XMLSchema#string"/>
  </owl:DatatypeProperty>
  <owl:DatatypeProperty rdf:about="http://example.org/onto/prop/google_data_loss_prevention_deidentify_template_integer_value">
    <rdfs:label>integer_value</rdfs:label>
    <rdfs:comment>An integer value (int64 format)</rdfs:comment>
    <rdfs:domain rdf:resource="http://example.org/onto/class/google_data_loss_prevention_deidentify_template"/>
    <rdfs:range rdf:resource="http://www.w3.org/2001/XMLSchema#string"/>
  </owl:DatatypeProperty>
  <owl:DatatypeProperty rdf:about="http://example.org/onto/prop/google_data_loss_prevention_deidentify_template_string_value">
    <rdfs:label>string_value</rdfs:label>
    <rdfs:comment>A string value.</rdfs:comment>
    <rdfs:domain rdf:resource="http://example.org/onto/class/google_data_loss_prevention_deidentify_template"/>
    <rdfs:range rdf:resource="http://www.w3.org/2001/XMLSchema#string"/>
  </owl:DatatypeProperty>
  <owl:DatatypeProperty rdf:about="http://example.org/onto/prop/google_data_loss_prevention_deidentify_template_timestamp_value">
    <rdfs:label>timestamp_value</rdfs:label>
    <rdfs:comment>A timestamp in RFC3339 UTC "Zulu" format, with nanosecond resolution and up to nine fractional digits. Examples: "2014-10-02T15:01:23Z" and "2014-10-02T15:01:23.045123456Z".</rdfs:comment>
    <rdfs:domain rdf:resource="http://example.org/onto/class/google_data_loss_prevention_deidentify_template"/>
    <rdfs:range rdf:resource="http://www.w3.org/2001/XMLSchema#string"/>
  </owl:DatatypeProperty>
  <owl:DatatypeProperty rdf:about="http://example.org/onto/prop/google_data_loss_prevention_deidentify_template_day">
    <rdfs:label>day</rdfs:label>
    <rdfs:comment>Day of a month. Must be from 1 to 31 and valid for the year and month, or 0 to specify a year by itself or a year and month where the day isn't significant.</rdfs:comment>
    <rdfs:domain rdf:resource="http://example.org/onto/class/google_data_loss_prevention_deidentify_template"/>
    <rdfs:range rdf:resource="http://www.w3.org/2001/XMLSchema#string"/>
  </owl:DatatypeProperty>
  <owl:DatatypeProperty rdf:about="http://example.org/onto/prop/google_data_loss_prevention_deidentify_template_month">
    <rdfs:label>month</rdfs:label>
    <rdfs:comment>Month of a year. Must be from 1 to 12, or 0 to specify a year without a month and day.</rdfs:comment>
    <rdfs:domain rdf:resource="http://example.org/onto/class/google_data_loss_prevention_deidentify_template"/>
    <rdfs:range rdf:resource="http://www.w3.org/2001/XMLSchema#string"/>
  </owl:DatatypeProperty>
  <owl:DatatypeProperty rdf:about="http://example.org/onto/prop/google_data_loss_prevention_deidentify_template_year">
    <rdfs:label>year</rdfs:label>
    <rdfs:comment>Year of the date. Must be from 1 to 9999, or 0 to specify a date without a year.</rdfs:comment>
    <rdfs:domain rdf:resource="http://example.org/onto/class/google_data_loss_prevention_deidentify_template"/>
    <rdfs:range rdf:resource="http://www.w3.org/2001/XMLSchema#string"/>
  </owl:DatatypeProperty>
  <owl:DatatypeProperty rdf:about="http://example.org/onto/prop/google_data_loss_prevention_deidentify_template_hours">
    <rdfs:label>hours</rdfs:label>
    <rdfs:comment>Hours of day in 24 hour format. Should be from 0 to 23. An API may choose to allow the value "24:00:00" for scenarios like business closing time.</rdfs:comment>
    <rdfs:domain rdf:resource="http://example.org/onto/class/google_data_loss_prevention_deidentify_template"/>
    <rdfs:range rdf:resource="http://www.w3.org/2001/XMLSchema#string"/>
  </owl:DatatypeProperty>
  <owl:DatatypeProperty rdf:about="http://example.org/onto/prop/google_data_loss_prevention_deidentify_template_minutes">
    <rdfs:label>minutes</rdfs:label>
    <rdfs:comment>Minutes of hour of day. Must be from 0 to 59.</rdfs:comment>
    <rdfs:domain rdf:resource="http://example.org/onto/class/google_data_loss_prevention_deidentify_template"/>
    <rdfs:range rdf:resource="http://www.w3.org/2001/XMLSchema#string"/>
  </owl:DatatypeProperty>
  <owl:DatatypeProperty rdf:about="http://example.org/onto/prop/google_data_loss_prevention_deidentify_template_nanos">
    <rdfs:label>nanos</rdfs:label>
    <rdfs:comment>Fractions of seconds in nanoseconds. Must be from 0 to 999,999,999.</rdfs:comment>
    <rdfs:domain rdf:resource="http://example.org/onto/class/google_data_loss_prevention_deidentify_template"/>
    <rdfs:range rdf:resource="http://www.w3.org/2001/XMLSchema#string"/>
  </owl:DatatypeProperty>
  <owl:DatatypeProperty rdf:about="http://example.org/onto/prop/google_data_loss_prevention_deidentify_template_seconds">
    <rdfs:label>seconds</rdfs:label>
    <rdfs:comment>Seconds of minutes of the time. Must normally be from 0 to 59. An API may allow the value 60 if it allows leap-seconds.</rdfs:comment>
    <rdfs:domain rdf:resource="http://example.org/onto/class/google_data_loss_prevention_deidentify_template"/>
    <rdfs:range rdf:resource="http://www.w3.org/2001/XMLSchema#string"/>
  </owl:DatatypeProperty>
  <owl:DatatypeProperty rdf:about="http://example.org/onto/prop/google_data_loss_prevention_deidentify_template_create">
    <rdfs:label>create</rdfs:label>
    <rdfs:domain rdf:resource="http://example.org/onto/class/google_data_loss_prevention_deidentify_template"/>
    <rdfs:range rdf:resource="http://www.w3.org/2001/XMLSchema#string"/>
  </owl:DatatypeProperty>
  <owl:DatatypeProperty rdf:about="http://example.org/onto/prop/google_data_loss_prevention_deidentify_template_delete">
    <rdfs:label>delete</rdfs:label>
    <rdfs:domain rdf:resource="http://example.org/onto/class/google_data_loss_prevention_deidentify_template"/>
    <rdfs:range rdf:resource="http://www.w3.org/2001/XMLSchema#string"/>
  </owl:DatatypeProperty>
  <owl:DatatypeProperty rdf:about="http://example.org/onto/prop/google_data_loss_prevention_deidentify_template_update">
    <rdfs:label>update</rdfs:label>
    <rdfs:domain rdf:resource="http://example.org/onto/class/google_data_loss_prevention_deidentify_template"/>
    <rdfs:range rdf:resource="http://www.w3.org/2001/XMLSchema#string"/>
  </owl:DatatypeProperty>
</rdf:RDF>
