<?xml version="1.0" encoding="UTF-8"?>
<rdf:RDF
  xmlns:rdf="http://www.w3.org/1999/02/22-rdf-syntax-ns#"
  xmlns:rdfs="http://www.w3.org/2000/01/rdf-schema#"
  xmlns:owl="http://www.w3.org/2002/07/owl#"
  xmlns:xsd="http://www.w3.org/2001/XMLSchema#"
  xml:base="http://example.org/onto/">
  <owl:Class rdf:about="http://example.org/onto/class/google_network_security_backend_authentication_config">
    <rdfs:label>google_network_security_backend_authentication_config</rdfs:label>
    <rdfs:comment>#
#     ***     AUTO GENERATED CODE    ***    Type: MMv1     ***
#
# ----------------------------------------------------------------------------
#
#     This code is generated by Magic Modules using the following:
#
#     Configuration: https:#github.com/GoogleCloudPlatform/magic-modules/tree/main/mmv1/products/networksecurity/BackendAuthenticationConfig.yaml
#     Template:      https:#github.com/GoogleCloudPlatform/magic-modules/tree/main/mmv1/templates/terraform/resource.html.markdown.tmpl
#
#     DO NOT EDIT this file directly. Any changes made to this file will be
#     overwritten during the next generation cycle.
#
# ----------------------------------------------------------------------------
subcategory: "Network Security"
description: |-
  BackendAuthenticationConfig groups the TrustConfig together with other settings that control how the load balancer authenticates, and expresses its identity to the backend.
---</rdfs:comment>
  </owl:Class>
  <owl:DatatypeProperty rdf:about="http://example.org/onto/prop/google_network_security_backend_authentication_config_client_certificate">
    <rdfs:label>client_certificate</rdfs:label>
    <rdfs:comment>Reference to a Certificate resource from the certificatemanager.googleapis.com namespace.
Used by a BackendService to negotiate mTLS when the backend connection uses TLS and the backend requests a client certificate. Must have a CLIENT_AUTH scope.</rdfs:comment>
    <rdfs:domain rdf:resource="http://example.org/onto/class/google_network_security_backend_authentication_config"/>
    <rdfs:range rdf:resource="http://www.w3.org/2001/XMLSchema#string"/>
  </owl:DatatypeProperty>
  <owl:DatatypeProperty rdf:about="http://example.org/onto/prop/google_network_security_backend_authentication_config_create_time">
    <rdfs:label>create_time</rdfs:label>
    <rdfs:comment>Time the BackendAuthenticationConfig was created in UTC.</rdfs:comment>
    <rdfs:domain rdf:resource="http://example.org/onto/class/google_network_security_backend_authentication_config"/>
    <rdfs:range rdf:resource="http://www.w3.org/2001/XMLSchema#string"/>
  </owl:DatatypeProperty>
  <owl:DatatypeProperty rdf:about="http://example.org/onto/prop/google_network_security_backend_authentication_config_description">
    <rdfs:label>description</rdfs:label>
    <rdfs:comment>A free-text description of the resource. Max length 1024 characters.</rdfs:comment>
    <rdfs:domain rdf:resource="http://example.org/onto/class/google_network_security_backend_authentication_config"/>
    <rdfs:range rdf:resource="http://www.w3.org/2001/XMLSchema#string"/>
  </owl:DatatypeProperty>
  <owl:DatatypeProperty rdf:about="http://example.org/onto/prop/google_network_security_backend_authentication_config_effective_labels">
    <rdfs:label>effective_labels</rdfs:label>
    <rdfs:comment>All of labels (key/value pairs) present on the resource in GCP, including the labels configured through Terraform, other clients and services.</rdfs:comment>
    <rdfs:domain rdf:resource="http://example.org/onto/class/google_network_security_backend_authentication_config"/>
    <rdfs:range rdf:resource="http://www.w3.org/2001/XMLSchema#string"/>
  </owl:DatatypeProperty>
  <owl:DatatypeProperty rdf:about="http://example.org/onto/prop/google_network_security_backend_authentication_config_id">
    <rdfs:label>id</rdfs:label>
    <rdfs:domain rdf:resource="http://example.org/onto/class/google_network_security_backend_authentication_config"/>
    <rdfs:range rdf:resource="http://www.w3.org/2001/XMLSchema#string"/>
  </owl:DatatypeProperty>
  <owl:DatatypeProperty rdf:about="http://example.org/onto/prop/google_network_security_backend_authentication_config_labels">
    <rdfs:label>labels</rdfs:label>
    <rdfs:comment>Set of label tags associated with the BackendAuthenticationConfig resource.

**Note**: This field is non-authoritative, and will only manage the labels present in your configuration.
Please refer to the field 'effective_labels' for all of the labels present on the resource.</rdfs:comment>
    <rdfs:domain rdf:resource="http://example.org/onto/class/google_network_security_backend_authentication_config"/>
    <rdfs:range rdf:resource="http://www.w3.org/2001/XMLSchema#string"/>
  </owl:DatatypeProperty>
  <owl:DatatypeProperty rdf:about="http://example.org/onto/prop/google_network_security_backend_authentication_config_location">
    <rdfs:label>location</rdfs:label>
    <rdfs:comment>The location of the backend authentication config.
The default value is 'global'.</rdfs:comment>
    <rdfs:domain rdf:resource="http://example.org/onto/class/google_network_security_backend_authentication_config"/>
    <rdfs:range rdf:resource="http://www.w3.org/2001/XMLSchema#string"/>
  </owl:DatatypeProperty>
  <owl:DatatypeProperty rdf:about="http://example.org/onto/prop/google_network_security_backend_authentication_config_name">
    <rdfs:label>name</rdfs:label>
    <rdfs:comment>Name of the BackendAuthenticationConfig resource.</rdfs:comment>
    <rdfs:domain rdf:resource="http://example.org/onto/class/google_network_security_backend_authentication_config"/>
    <rdfs:range rdf:resource="http://www.w3.org/2001/XMLSchema#string"/>
  </owl:DatatypeProperty>
  <owl:DatatypeProperty rdf:about="http://example.org/onto/prop/google_network_security_backend_authentication_config_project">
    <rdfs:label>project</rdfs:label>
    <rdfs:domain rdf:resource="http://example.org/onto/class/google_network_security_backend_authentication_config"/>
    <rdfs:range rdf:resource="http://www.w3.org/2001/XMLSchema#string"/>
  </owl:DatatypeProperty>
  <owl:DatatypeProperty rdf:about="http://example.org/onto/prop/google_network_security_backend_authentication_config_terraform_labels">
    <rdfs:label>terraform_labels</rdfs:label>
    <rdfs:comment>The combination of labels configured directly on the resource
 and default labels configured on the provider.</rdfs:comment>
    <rdfs:domain rdf:resource="http://example.org/onto/class/google_network_security_backend_authentication_config"/>
    <rdfs:range rdf:resource="http://www.w3.org/2001/XMLSchema#string"/>
  </owl:DatatypeProperty>
  <owl:DatatypeProperty rdf:about="http://example.org/onto/prop/google_network_security_backend_authentication_config_trust_config">
    <rdfs:label>trust_config</rdfs:label>
    <rdfs:comment>Reference to a TrustConfig resource from the certificatemanager.googleapis.com namespace.
A BackendService uses the chain of trust represented by this TrustConfig, if specified, to validate the server certificates presented by the backend. Required unless wellKnownRoots is set to PUBLIC_ROOTS.</rdfs:comment>
    <rdfs:domain rdf:resource="http://example.org/onto/class/google_network_security_backend_authentication_config"/>
    <rdfs:range rdf:resource="http://www.w3.org/2001/XMLSchema#string"/>
  </owl:DatatypeProperty>
  <owl:DatatypeProperty rdf:about="http://example.org/onto/prop/google_network_security_backend_authentication_config_update_time">
    <rdfs:label>update_time</rdfs:label>
    <rdfs:comment>Time the BackendAuthenticationConfig was updated in UTC.</rdfs:comment>
    <rdfs:domain rdf:resource="http://example.org/onto/class/google_network_security_backend_authentication_config"/>
    <rdfs:range rdf:resource="http://www.w3.org/2001/XMLSchema#string"/>
  </owl:DatatypeProperty>
  <owl:DatatypeProperty rdf:about="http://example.org/onto/prop/google_network_security_backend_authentication_config_well_known_roots">
    <rdfs:label>well_known_roots</rdfs:label>
    <rdfs:comment>Well known roots to use for server certificate validation. If set to NONE, the BackendService will only validate server certificates against roots specified in TrustConfig.
If set to PUBLIC_ROOTS, the BackendService uses a set of well-known public roots, in addition to any roots specified in the trustConfig field, when validating the server certificates presented by the backend.
Validation with these roots is only considered when the TlsSettings.sni field in the BackendService is set. The well-known roots are a set of root CAs managed by Google. CAs in this set can be added or removed without notice. Possible values: ["NONE", "PUBLIC_ROOTS"]</rdfs:comment>
    <rdfs:domain rdf:resource="http://example.org/onto/class/google_network_security_backend_authentication_config"/>
    <rdfs:range rdf:resource="http://www.w3.org/2001/XMLSchema#string"/>
  </owl:DatatypeProperty>
  <owl:DatatypeProperty rdf:about="http://example.org/onto/prop/google_network_security_backend_authentication_config_create">
    <rdfs:label>create</rdfs:label>
    <rdfs:domain rdf:resource="http://example.org/onto/class/google_network_security_backend_authentication_config"/>
    <rdfs:range rdf:resource="http://www.w3.org/2001/XMLSchema#string"/>
  </owl:DatatypeProperty>
  <owl:DatatypeProperty rdf:about="http://example.org/onto/prop/google_network_security_backend_authentication_config_delete">
    <rdfs:label>delete</rdfs:label>
    <rdfs:domain rdf:resource="http://example.org/onto/class/google_network_security_backend_authentication_config"/>
    <rdfs:range rdf:resource="http://www.w3.org/2001/XMLSchema#string"/>
  </owl:DatatypeProperty>
  <owl:DatatypeProperty rdf:about="http://example.org/onto/prop/google_network_security_backend_authentication_config_update">
    <rdfs:label>update</rdfs:label>
    <rdfs:domain rdf:resource="http://example.org/onto/class/google_network_security_backend_authentication_config"/>
    <rdfs:range rdf:resource="http://www.w3.org/2001/XMLSchema#string"/>
  </owl:DatatypeProperty>
</rdf:RDF>
