<?xml version="1.0" encoding="UTF-8"?>
<rdf:RDF
  xmlns:rdf="http://www.w3.org/1999/02/22-rdf-syntax-ns#"
  xmlns:rdfs="http://www.w3.org/2000/01/rdf-schema#"
  xmlns:owl="http://www.w3.org/2002/07/owl#"
  xmlns:xsd="http://www.w3.org/2001/XMLSchema#"
  xml:base="http://example.org/onto/">
  <owl:Class rdf:about="http://example.org/onto/class/google_apigee_instance">
    <rdfs:label>google_apigee_instance</rdfs:label>
    <rdfs:comment>#
#     ***     AUTO GENERATED CODE    ***    Type: MMv1     ***
#
# ----------------------------------------------------------------------------
#
#     This code is generated by Magic Modules using the following:
#
#     Configuration: https:#github.com/GoogleCloudPlatform/magic-modules/tree/main/mmv1/products/apigee/Instance.yaml
#     Template:      https:#github.com/GoogleCloudPlatform/magic-modules/tree/main/mmv1/templates/terraform/resource.html.markdown.tmpl
#
#     DO NOT EDIT this file directly. Any changes made to this file will be
#     overwritten during the next generation cycle.
#
# ----------------------------------------------------------------------------
subcategory: "Apigee"
description: |-
  An `Instance` is the runtime dataplane in Apigee.
---</rdfs:comment>
  </owl:Class>
  <owl:DatatypeProperty rdf:about="http://example.org/onto/prop/google_apigee_instance_consumer_accept_list">
    <rdfs:label>consumer_accept_list</rdfs:label>
    <rdfs:comment>Optional. Customer accept list represents the list of projects (id/number) on customer
side that can privately connect to the service attachment. It is an optional field
which the customers can provide during the instance creation. By default, the customer
project associated with the Apigee organization will be included to the list.</rdfs:comment>
    <rdfs:domain rdf:resource="http://example.org/onto/class/google_apigee_instance"/>
    <rdfs:range rdf:resource="http://www.w3.org/2001/XMLSchema#string"/>
  </owl:DatatypeProperty>
  <owl:DatatypeProperty rdf:about="http://example.org/onto/prop/google_apigee_instance_description">
    <rdfs:label>description</rdfs:label>
    <rdfs:comment>Description of the instance.</rdfs:comment>
    <rdfs:domain rdf:resource="http://example.org/onto/class/google_apigee_instance"/>
    <rdfs:range rdf:resource="http://www.w3.org/2001/XMLSchema#string"/>
  </owl:DatatypeProperty>
  <owl:DatatypeProperty rdf:about="http://example.org/onto/prop/google_apigee_instance_disk_encryption_key_name">
    <rdfs:label>disk_encryption_key_name</rdfs:label>
    <rdfs:comment>Customer Managed Encryption Key (CMEK) used for disk and volume encryption. Required for Apigee paid subscriptions only.
Use the following format: 'projects/([^/]+)/locations/([^/]+)/keyRings/([^/]+)/cryptoKeys/([^/]+)'</rdfs:comment>
    <rdfs:domain rdf:resource="http://example.org/onto/class/google_apigee_instance"/>
    <rdfs:range rdf:resource="http://www.w3.org/2001/XMLSchema#string"/>
  </owl:DatatypeProperty>
  <owl:DatatypeProperty rdf:about="http://example.org/onto/prop/google_apigee_instance_display_name">
    <rdfs:label>display_name</rdfs:label>
    <rdfs:comment>Display name of the instance.</rdfs:comment>
    <rdfs:domain rdf:resource="http://example.org/onto/class/google_apigee_instance"/>
    <rdfs:range rdf:resource="http://www.w3.org/2001/XMLSchema#string"/>
  </owl:DatatypeProperty>
  <owl:DatatypeProperty rdf:about="http://example.org/onto/prop/google_apigee_instance_host">
    <rdfs:label>host</rdfs:label>
    <rdfs:comment>Output only. Hostname or IP address of the exposed Apigee endpoint used by clients to connect to the service.</rdfs:comment>
    <rdfs:domain rdf:resource="http://example.org/onto/class/google_apigee_instance"/>
    <rdfs:range rdf:resource="http://www.w3.org/2001/XMLSchema#string"/>
  </owl:DatatypeProperty>
  <owl:DatatypeProperty rdf:about="http://example.org/onto/prop/google_apigee_instance_id">
    <rdfs:label>id</rdfs:label>
    <rdfs:domain rdf:resource="http://example.org/onto/class/google_apigee_instance"/>
    <rdfs:range rdf:resource="http://www.w3.org/2001/XMLSchema#string"/>
  </owl:DatatypeProperty>
  <owl:DatatypeProperty rdf:about="http://example.org/onto/prop/google_apigee_instance_ip_range">
    <rdfs:label>ip_range</rdfs:label>
    <rdfs:comment>IP range represents the customer-provided CIDR block of length 22 that will be used for
the Apigee instance creation. This optional range, if provided, should be freely
available as part of larger named range the customer has allocated to the Service
Networking peering. If this is not provided, Apigee will automatically request for any
available /22 CIDR block from Service Networking. The customer should use this CIDR block
for configuring their firewall needs to allow traffic from Apigee.
Input format: "a.b.c.d/22"</rdfs:comment>
    <rdfs:domain rdf:resource="http://example.org/onto/class/google_apigee_instance"/>
    <rdfs:range rdf:resource="http://www.w3.org/2001/XMLSchema#string"/>
  </owl:DatatypeProperty>
  <owl:DatatypeProperty rdf:about="http://example.org/onto/prop/google_apigee_instance_location">
    <rdfs:label>location</rdfs:label>
    <rdfs:comment>Required. Compute Engine location where the instance resides.</rdfs:comment>
    <rdfs:domain rdf:resource="http://example.org/onto/class/google_apigee_instance"/>
    <rdfs:range rdf:resource="http://www.w3.org/2001/XMLSchema#string"/>
  </owl:DatatypeProperty>
  <owl:DatatypeProperty rdf:about="http://example.org/onto/prop/google_apigee_instance_name">
    <rdfs:label>name</rdfs:label>
    <rdfs:comment>Resource ID of the instance.</rdfs:comment>
    <rdfs:domain rdf:resource="http://example.org/onto/class/google_apigee_instance"/>
    <rdfs:range rdf:resource="http://www.w3.org/2001/XMLSchema#string"/>
  </owl:DatatypeProperty>
  <owl:DatatypeProperty rdf:about="http://example.org/onto/prop/google_apigee_instance_org_id">
    <rdfs:label>org_id</rdfs:label>
    <rdfs:comment>The Apigee Organization associated with the Apigee instance,
in the format 'organizations/{{org_name}}'.</rdfs:comment>
    <rdfs:domain rdf:resource="http://example.org/onto/class/google_apigee_instance"/>
    <rdfs:range rdf:resource="http://www.w3.org/2001/XMLSchema#string"/>
  </owl:DatatypeProperty>
  <owl:DatatypeProperty rdf:about="http://example.org/onto/prop/google_apigee_instance_peering_cidr_range">
    <rdfs:label>peering_cidr_range</rdfs:label>
    <rdfs:comment>The size of the CIDR block range that will be reserved by the instance. For valid values,
see [CidrRange](https://cloud.google.com/apigee/docs/reference/apis/apigee/rest/v1/organizations.instances#CidrRange) on the documentation.</rdfs:comment>
    <rdfs:domain rdf:resource="http://example.org/onto/class/google_apigee_instance"/>
    <rdfs:range rdf:resource="http://www.w3.org/2001/XMLSchema#string"/>
  </owl:DatatypeProperty>
  <owl:DatatypeProperty rdf:about="http://example.org/onto/prop/google_apigee_instance_port">
    <rdfs:label>port</rdfs:label>
    <rdfs:comment>Output only. Port number of the exposed Apigee endpoint.</rdfs:comment>
    <rdfs:domain rdf:resource="http://example.org/onto/class/google_apigee_instance"/>
    <rdfs:range rdf:resource="http://www.w3.org/2001/XMLSchema#string"/>
  </owl:DatatypeProperty>
  <owl:DatatypeProperty rdf:about="http://example.org/onto/prop/google_apigee_instance_service_attachment">
    <rdfs:label>service_attachment</rdfs:label>
    <rdfs:comment>Output only. Resource name of the service attachment created for the instance in
the format: projects/*/regions/*/serviceAttachments/* Apigee customers can privately
forward traffic to this service attachment using the PSC endpoints.</rdfs:comment>
    <rdfs:domain rdf:resource="http://example.org/onto/class/google_apigee_instance"/>
    <rdfs:range rdf:resource="http://www.w3.org/2001/XMLSchema#string"/>
  </owl:DatatypeProperty>
  <owl:DatatypeProperty rdf:about="http://example.org/onto/prop/google_apigee_instance_enabled">
    <rdfs:label>enabled</rdfs:label>
    <rdfs:comment>Boolean flag that specifies whether the customer access log feature is enabled.</rdfs:comment>
    <rdfs:domain rdf:resource="http://example.org/onto/class/google_apigee_instance"/>
    <rdfs:range rdf:resource="http://www.w3.org/2001/XMLSchema#string"/>
  </owl:DatatypeProperty>
  <owl:DatatypeProperty rdf:about="http://example.org/onto/prop/google_apigee_instance_filter">
    <rdfs:label>filter</rdfs:label>
    <rdfs:comment>Ship the access log entries that match the statusCode defined in the filter.
The statusCode is the only expected/supported filter field. (Ex: statusCode)
The filter will parse it to the Common Expression Language semantics for expression
evaluation to build the filter condition. (Ex: "filter": statusCode >= 200 && statusCode < 300 )</rdfs:comment>
    <rdfs:domain rdf:resource="http://example.org/onto/class/google_apigee_instance"/>
    <rdfs:range rdf:resource="http://www.w3.org/2001/XMLSchema#string"/>
  </owl:DatatypeProperty>
  <owl:DatatypeProperty rdf:about="http://example.org/onto/prop/google_apigee_instance_create">
    <rdfs:label>create</rdfs:label>
    <rdfs:domain rdf:resource="http://example.org/onto/class/google_apigee_instance"/>
    <rdfs:range rdf:resource="http://www.w3.org/2001/XMLSchema#string"/>
  </owl:DatatypeProperty>
  <owl:DatatypeProperty rdf:about="http://example.org/onto/prop/google_apigee_instance_delete">
    <rdfs:label>delete</rdfs:label>
    <rdfs:domain rdf:resource="http://example.org/onto/class/google_apigee_instance"/>
    <rdfs:range rdf:resource="http://www.w3.org/2001/XMLSchema#string"/>
  </owl:DatatypeProperty>
  <owl:DatatypeProperty rdf:about="http://example.org/onto/prop/google_apigee_instance_update">
    <rdfs:label>update</rdfs:label>
    <rdfs:domain rdf:resource="http://example.org/onto/class/google_apigee_instance"/>
    <rdfs:range rdf:resource="http://www.w3.org/2001/XMLSchema#string"/>
  </owl:DatatypeProperty>
</rdf:RDF>
