<?xml version="1.0" encoding="UTF-8"?>
<rdf:RDF
  xmlns:rdf="http://www.w3.org/1999/02/22-rdf-syntax-ns#"
  xmlns:rdfs="http://www.w3.org/2000/01/rdf-schema#"
  xmlns:owl="http://www.w3.org/2002/07/owl#"
  xmlns:xsd="http://www.w3.org/2001/XMLSchema#"
  xml:base="http://example.org/onto/">
  <owl:Class rdf:about="http://example.org/onto/class/google_managed_kafka_topic">
    <rdfs:label>google_managed_kafka_topic</rdfs:label>
    <rdfs:comment>#
#     ***     AUTO GENERATED CODE    ***    Type: MMv1     ***
#
# ----------------------------------------------------------------------------
#
#     This code is generated by Magic Modules using the following:
#
#     Configuration: https:#github.com/GoogleCloudPlatform/magic-modules/tree/main/mmv1/products/managedkafka/Topic.yaml
#     Template:      https:#github.com/GoogleCloudPlatform/magic-modules/tree/main/mmv1/templates/terraform/resource.html.markdown.tmpl
#
#     DO NOT EDIT this file directly. Any changes made to this file will be
#     overwritten during the next generation cycle.
#
# ----------------------------------------------------------------------------
subcategory: "Managed Kafka"
description: |-
  A Managed Service for Apache Kafka topic.
---</rdfs:comment>
  </owl:Class>
  <owl:DatatypeProperty rdf:about="http://example.org/onto/prop/google_managed_kafka_topic_cluster">
    <rdfs:label>cluster</rdfs:label>
    <rdfs:comment>The cluster name.</rdfs:comment>
    <rdfs:domain rdf:resource="http://example.org/onto/class/google_managed_kafka_topic"/>
    <rdfs:range rdf:resource="http://www.w3.org/2001/XMLSchema#string"/>
  </owl:DatatypeProperty>
  <owl:DatatypeProperty rdf:about="http://example.org/onto/prop/google_managed_kafka_topic_configs">
    <rdfs:label>configs</rdfs:label>
    <rdfs:comment>Configuration for the topic that are overridden from the cluster defaults. The key of the map is a Kafka topic property name, for example: 'cleanup.policy=compact', 'compression.type=producer'.</rdfs:comment>
    <rdfs:domain rdf:resource="http://example.org/onto/class/google_managed_kafka_topic"/>
    <rdfs:range rdf:resource="http://www.w3.org/2001/XMLSchema#string"/>
  </owl:DatatypeProperty>
  <owl:DatatypeProperty rdf:about="http://example.org/onto/prop/google_managed_kafka_topic_id">
    <rdfs:label>id</rdfs:label>
    <rdfs:domain rdf:resource="http://example.org/onto/class/google_managed_kafka_topic"/>
    <rdfs:range rdf:resource="http://www.w3.org/2001/XMLSchema#string"/>
  </owl:DatatypeProperty>
  <owl:DatatypeProperty rdf:about="http://example.org/onto/prop/google_managed_kafka_topic_location">
    <rdfs:label>location</rdfs:label>
    <rdfs:comment>ID of the location of the Kafka resource. See https://cloud.google.com/managed-kafka/docs/locations for a list of supported locations.</rdfs:comment>
    <rdfs:domain rdf:resource="http://example.org/onto/class/google_managed_kafka_topic"/>
    <rdfs:range rdf:resource="http://www.w3.org/2001/XMLSchema#string"/>
  </owl:DatatypeProperty>
  <owl:DatatypeProperty rdf:about="http://example.org/onto/prop/google_managed_kafka_topic_name">
    <rdfs:label>name</rdfs:label>
    <rdfs:comment>The name of the topic. The 'topic' segment is used when connecting directly to the cluster. Must be in the format 'projects/PROJECT_ID/locations/LOCATION/clusters/CLUSTER_ID/topics/TOPIC_ID'.</rdfs:comment>
    <rdfs:domain rdf:resource="http://example.org/onto/class/google_managed_kafka_topic"/>
    <rdfs:range rdf:resource="http://www.w3.org/2001/XMLSchema#string"/>
  </owl:DatatypeProperty>
  <owl:DatatypeProperty rdf:about="http://example.org/onto/prop/google_managed_kafka_topic_partition_count">
    <rdfs:label>partition_count</rdfs:label>
    <rdfs:comment>The number of partitions in a topic. You can increase the partition count for a topic, but you cannot decrease it. Increasing partitions for a topic that uses a key might change how messages are distributed.</rdfs:comment>
    <rdfs:domain rdf:resource="http://example.org/onto/class/google_managed_kafka_topic"/>
    <rdfs:range rdf:resource="http://www.w3.org/2001/XMLSchema#string"/>
  </owl:DatatypeProperty>
  <owl:DatatypeProperty rdf:about="http://example.org/onto/prop/google_managed_kafka_topic_project">
    <rdfs:label>project</rdfs:label>
    <rdfs:domain rdf:resource="http://example.org/onto/class/google_managed_kafka_topic"/>
    <rdfs:range rdf:resource="http://www.w3.org/2001/XMLSchema#string"/>
  </owl:DatatypeProperty>
  <owl:DatatypeProperty rdf:about="http://example.org/onto/prop/google_managed_kafka_topic_replication_factor">
    <rdfs:label>replication_factor</rdfs:label>
    <rdfs:comment>The number of replicas of each partition. A replication factor of 3 is recommended for high availability.</rdfs:comment>
    <rdfs:domain rdf:resource="http://example.org/onto/class/google_managed_kafka_topic"/>
    <rdfs:range rdf:resource="http://www.w3.org/2001/XMLSchema#string"/>
  </owl:DatatypeProperty>
  <owl:DatatypeProperty rdf:about="http://example.org/onto/prop/google_managed_kafka_topic_topic_id">
    <rdfs:label>topic_id</rdfs:label>
    <rdfs:comment>The ID to use for the topic, which will become the final component of the topic's name. This value is structured like: 'my-topic-name'.</rdfs:comment>
    <rdfs:domain rdf:resource="http://example.org/onto/class/google_managed_kafka_topic"/>
    <rdfs:range rdf:resource="http://www.w3.org/2001/XMLSchema#string"/>
  </owl:DatatypeProperty>
  <owl:DatatypeProperty rdf:about="http://example.org/onto/prop/google_managed_kafka_topic_create">
    <rdfs:label>create</rdfs:label>
    <rdfs:domain rdf:resource="http://example.org/onto/class/google_managed_kafka_topic"/>
    <rdfs:range rdf:resource="http://www.w3.org/2001/XMLSchema#string"/>
  </owl:DatatypeProperty>
  <owl:DatatypeProperty rdf:about="http://example.org/onto/prop/google_managed_kafka_topic_delete">
    <rdfs:label>delete</rdfs:label>
    <rdfs:domain rdf:resource="http://example.org/onto/class/google_managed_kafka_topic"/>
    <rdfs:range rdf:resource="http://www.w3.org/2001/XMLSchema#string"/>
  </owl:DatatypeProperty>
  <owl:DatatypeProperty rdf:about="http://example.org/onto/prop/google_managed_kafka_topic_update">
    <rdfs:label>update</rdfs:label>
    <rdfs:domain rdf:resource="http://example.org/onto/class/google_managed_kafka_topic"/>
    <rdfs:range rdf:resource="http://www.w3.org/2001/XMLSchema#string"/>
  </owl:DatatypeProperty>
</rdf:RDF>
