<?xml version="1.0" encoding="UTF-8"?>
<rdf:RDF
  xmlns:rdf="http://www.w3.org/1999/02/22-rdf-syntax-ns#"
  xmlns:rdfs="http://www.w3.org/2000/01/rdf-schema#"
  xmlns:owl="http://www.w3.org/2002/07/owl#"
  xmlns:xsd="http://www.w3.org/2001/XMLSchema#"
  xml:base="http://example.org/onto/">
  <owl:Class rdf:about="http://example.org/onto/class/google_compute_network_endpoint">
    <rdfs:label>google_compute_network_endpoint</rdfs:label>
    <rdfs:comment>#
#     ***     AUTO GENERATED CODE    ***    Type: MMv1     ***
#
# ----------------------------------------------------------------------------
#
#     This code is generated by Magic Modules using the following:
#
#     Configuration: https:#github.com/GoogleCloudPlatform/magic-modules/tree/main/mmv1/products/compute/NetworkEndpoint.yaml
#     Template:      https:#github.com/GoogleCloudPlatform/magic-modules/tree/main/mmv1/templates/terraform/resource.html.markdown.tmpl
#
#     DO NOT EDIT this file directly. Any changes made to this file will be
#     overwritten during the next generation cycle.
#
# ----------------------------------------------------------------------------
subcategory: "Compute Engine"
description: |-
  A Network endpoint represents a IP address and port combination that is
  part of a specific network endpoint group (NEG).
---</rdfs:comment>
  </owl:Class>
  <owl:DatatypeProperty rdf:about="http://example.org/onto/prop/google_compute_network_endpoint_id">
    <rdfs:label>id</rdfs:label>
    <rdfs:domain rdf:resource="http://example.org/onto/class/google_compute_network_endpoint"/>
    <rdfs:range rdf:resource="http://www.w3.org/2001/XMLSchema#string"/>
  </owl:DatatypeProperty>
  <owl:DatatypeProperty rdf:about="http://example.org/onto/prop/google_compute_network_endpoint_instance">
    <rdfs:label>instance</rdfs:label>
    <rdfs:comment>The name for a specific VM instance that the IP address belongs to.
This is required for network endpoints of type GCE_VM_IP_PORT.
The instance must be in the same zone of network endpoint group.</rdfs:comment>
    <rdfs:domain rdf:resource="http://example.org/onto/class/google_compute_network_endpoint"/>
    <rdfs:range rdf:resource="http://www.w3.org/2001/XMLSchema#string"/>
  </owl:DatatypeProperty>
  <owl:DatatypeProperty rdf:about="http://example.org/onto/prop/google_compute_network_endpoint_ip_address">
    <rdfs:label>ip_address</rdfs:label>
    <rdfs:comment>IPv4 address of network endpoint. The IP address must belong
to a VM in GCE (either the primary IP or as part of an aliased IP
range).</rdfs:comment>
    <rdfs:domain rdf:resource="http://example.org/onto/class/google_compute_network_endpoint"/>
    <rdfs:range rdf:resource="http://www.w3.org/2001/XMLSchema#string"/>
  </owl:DatatypeProperty>
  <owl:DatatypeProperty rdf:about="http://example.org/onto/prop/google_compute_network_endpoint_network_endpoint_group">
    <rdfs:label>network_endpoint_group</rdfs:label>
    <rdfs:comment>The network endpoint group this endpoint is part of.</rdfs:comment>
    <rdfs:domain rdf:resource="http://example.org/onto/class/google_compute_network_endpoint"/>
    <rdfs:range rdf:resource="http://www.w3.org/2001/XMLSchema#string"/>
  </owl:DatatypeProperty>
  <owl:DatatypeProperty rdf:about="http://example.org/onto/prop/google_compute_network_endpoint_port">
    <rdfs:label>port</rdfs:label>
    <rdfs:comment>Port number of network endpoint.
**Note** 'port' is required unless the Network Endpoint Group is created
with the type of 'GCE_VM_IP'</rdfs:comment>
    <rdfs:domain rdf:resource="http://example.org/onto/class/google_compute_network_endpoint"/>
    <rdfs:range rdf:resource="http://www.w3.org/2001/XMLSchema#string"/>
  </owl:DatatypeProperty>
  <owl:DatatypeProperty rdf:about="http://example.org/onto/prop/google_compute_network_endpoint_project">
    <rdfs:label>project</rdfs:label>
    <rdfs:domain rdf:resource="http://example.org/onto/class/google_compute_network_endpoint"/>
    <rdfs:range rdf:resource="http://www.w3.org/2001/XMLSchema#string"/>
  </owl:DatatypeProperty>
  <owl:DatatypeProperty rdf:about="http://example.org/onto/prop/google_compute_network_endpoint_zone">
    <rdfs:label>zone</rdfs:label>
    <rdfs:comment>Zone where the containing network endpoint group is located.</rdfs:comment>
    <rdfs:domain rdf:resource="http://example.org/onto/class/google_compute_network_endpoint"/>
    <rdfs:range rdf:resource="http://www.w3.org/2001/XMLSchema#string"/>
  </owl:DatatypeProperty>
  <owl:DatatypeProperty rdf:about="http://example.org/onto/prop/google_compute_network_endpoint_create">
    <rdfs:label>create</rdfs:label>
    <rdfs:domain rdf:resource="http://example.org/onto/class/google_compute_network_endpoint"/>
    <rdfs:range rdf:resource="http://www.w3.org/2001/XMLSchema#string"/>
  </owl:DatatypeProperty>
  <owl:DatatypeProperty rdf:about="http://example.org/onto/prop/google_compute_network_endpoint_delete">
    <rdfs:label>delete</rdfs:label>
    <rdfs:domain rdf:resource="http://example.org/onto/class/google_compute_network_endpoint"/>
    <rdfs:range rdf:resource="http://www.w3.org/2001/XMLSchema#string"/>
  </owl:DatatypeProperty>
</rdf:RDF>
