<?xml version="1.0" encoding="UTF-8"?>
<rdf:RDF
  xmlns:rdf="http://www.w3.org/1999/02/22-rdf-syntax-ns#"
  xmlns:rdfs="http://www.w3.org/2000/01/rdf-schema#"
  xmlns:owl="http://www.w3.org/2002/07/owl#"
  xmlns:xsd="http://www.w3.org/2001/XMLSchema#"
  xml:base="http://example.org/onto/">
  <owl:Class rdf:about="http://example.org/onto/class/google_spanner_instance">
    <rdfs:label>google_spanner_instance</rdfs:label>
    <rdfs:comment>#
#     ***     AUTO GENERATED CODE    ***    Type: MMv1     ***
#
# ----------------------------------------------------------------------------
#
#     This code is generated by Magic Modules using the following:
#
#     Configuration: https:#github.com/GoogleCloudPlatform/magic-modules/tree/main/mmv1/products/spanner/Instance.yaml
#     Template:      https:#github.com/GoogleCloudPlatform/magic-modules/tree/main/mmv1/templates/terraform/resource.html.markdown.tmpl
#
#     DO NOT EDIT this file directly. Any changes made to this file will be
#     overwritten during the next generation cycle.
#
# ----------------------------------------------------------------------------
subcategory: "Cloud Spanner"
description: |-
  An isolated set of Cloud Spanner resources on which databases can be
  hosted.
---</rdfs:comment>
  </owl:Class>
  <owl:DatatypeProperty rdf:about="http://example.org/onto/prop/google_spanner_instance_config">
    <rdfs:label>config</rdfs:label>
    <rdfs:comment>The name of the instance's configuration (similar but not
quite the same as a region) which defines the geographic placement and
replication of your databases in this instance. It determines where your data
is stored. Values are typically of the form 'regional-europe-west1' , 'us-central' etc.
In order to obtain a valid list please consult the
[Configuration section of the docs](https://cloud.google.com/spanner/docs/instances).</rdfs:comment>
    <rdfs:domain rdf:resource="http://example.org/onto/class/google_spanner_instance"/>
    <rdfs:range rdf:resource="http://www.w3.org/2001/XMLSchema#string"/>
  </owl:DatatypeProperty>
  <owl:DatatypeProperty rdf:about="http://example.org/onto/prop/google_spanner_instance_default_backup_schedule_type">
    <rdfs:label>default_backup_schedule_type</rdfs:label>
    <rdfs:comment>Controls the default backup behavior for new databases within the instance.
Note that 'AUTOMATIC' is not permitted for free instances, as backups and backup schedules are not allowed for free instances.
if unset or NONE, no default backup schedule will be created for new databases within the instance. Possible values: ["NONE", "AUTOMATIC"]</rdfs:comment>
    <rdfs:domain rdf:resource="http://example.org/onto/class/google_spanner_instance"/>
    <rdfs:range rdf:resource="http://www.w3.org/2001/XMLSchema#string"/>
  </owl:DatatypeProperty>
  <owl:DatatypeProperty rdf:about="http://example.org/onto/prop/google_spanner_instance_display_name">
    <rdfs:label>display_name</rdfs:label>
    <rdfs:comment>The descriptive name for this instance as it appears in UIs. Must be
unique per project and between 4 and 30 characters in length.</rdfs:comment>
    <rdfs:domain rdf:resource="http://example.org/onto/class/google_spanner_instance"/>
    <rdfs:range rdf:resource="http://www.w3.org/2001/XMLSchema#string"/>
  </owl:DatatypeProperty>
  <owl:DatatypeProperty rdf:about="http://example.org/onto/prop/google_spanner_instance_edition">
    <rdfs:label>edition</rdfs:label>
    <rdfs:comment>The edition selected for this instance. Different editions provide different capabilities at different price points. Possible values: ["EDITION_UNSPECIFIED", "STANDARD", "ENTERPRISE", "ENTERPRISE_PLUS"]</rdfs:comment>
    <rdfs:domain rdf:resource="http://example.org/onto/class/google_spanner_instance"/>
    <rdfs:range rdf:resource="http://www.w3.org/2001/XMLSchema#string"/>
  </owl:DatatypeProperty>
  <owl:DatatypeProperty rdf:about="http://example.org/onto/prop/google_spanner_instance_effective_labels">
    <rdfs:label>effective_labels</rdfs:label>
    <rdfs:comment>All of labels (key/value pairs) present on the resource in GCP, including the labels configured through Terraform, other clients and services.</rdfs:comment>
    <rdfs:domain rdf:resource="http://example.org/onto/class/google_spanner_instance"/>
    <rdfs:range rdf:resource="http://www.w3.org/2001/XMLSchema#string"/>
  </owl:DatatypeProperty>
  <owl:DatatypeProperty rdf:about="http://example.org/onto/prop/google_spanner_instance_force_destroy">
    <rdfs:label>force_destroy</rdfs:label>
    <rdfs:comment>When deleting a spanner instance, this boolean option will delete all backups of this instance.
This must be set to true if you created a backup manually in the console.</rdfs:comment>
    <rdfs:domain rdf:resource="http://example.org/onto/class/google_spanner_instance"/>
    <rdfs:range rdf:resource="http://www.w3.org/2001/XMLSchema#string"/>
  </owl:DatatypeProperty>
  <owl:DatatypeProperty rdf:about="http://example.org/onto/prop/google_spanner_instance_id">
    <rdfs:label>id</rdfs:label>
    <rdfs:domain rdf:resource="http://example.org/onto/class/google_spanner_instance"/>
    <rdfs:range rdf:resource="http://www.w3.org/2001/XMLSchema#string"/>
  </owl:DatatypeProperty>
  <owl:DatatypeProperty rdf:about="http://example.org/onto/prop/google_spanner_instance_instance_type">
    <rdfs:label>instance_type</rdfs:label>
    <rdfs:comment>The type of this instance. The type can be used to distinguish product variants, that can affect aspects like:
usage restrictions, quotas and billing. Currently this is used to distinguish FREE_INSTANCE vs PROVISIONED instances.
When configured as FREE_INSTANCE, the field 'edition' should not be configured. Possible values: ["PROVISIONED", "FREE_INSTANCE"]</rdfs:comment>
    <rdfs:domain rdf:resource="http://example.org/onto/class/google_spanner_instance"/>
    <rdfs:range rdf:resource="http://www.w3.org/2001/XMLSchema#string"/>
  </owl:DatatypeProperty>
  <owl:DatatypeProperty rdf:about="http://example.org/onto/prop/google_spanner_instance_labels">
    <rdfs:label>labels</rdfs:label>
    <rdfs:comment>An object containing a list of "key": value pairs.
Example: { "name": "wrench", "mass": "1.3kg", "count": "3" }.


**Note**: This field is non-authoritative, and will only manage the labels present in your configuration.
Please refer to the field 'effective_labels' for all of the labels present on the resource.</rdfs:comment>
    <rdfs:domain rdf:resource="http://example.org/onto/class/google_spanner_instance"/>
    <rdfs:range rdf:resource="http://www.w3.org/2001/XMLSchema#string"/>
  </owl:DatatypeProperty>
  <owl:DatatypeProperty rdf:about="http://example.org/onto/prop/google_spanner_instance_name">
    <rdfs:label>name</rdfs:label>
    <rdfs:comment>A unique identifier for the instance, which cannot be changed after
the instance is created. The name must be between 6 and 30 characters
in length.
If not provided, a random string starting with 'tf-' will be selected.</rdfs:comment>
    <rdfs:domain rdf:resource="http://example.org/onto/class/google_spanner_instance"/>
    <rdfs:range rdf:resource="http://www.w3.org/2001/XMLSchema#string"/>
  </owl:DatatypeProperty>
  <owl:DatatypeProperty rdf:about="http://example.org/onto/prop/google_spanner_instance_num_nodes">
    <rdfs:label>num_nodes</rdfs:label>
    <rdfs:comment>The number of nodes allocated to this instance. Exactly one of either num_nodes, processing_units or
autoscaling_config must be present in terraform except when instance_type = FREE_INSTANCE.</rdfs:comment>
    <rdfs:domain rdf:resource="http://example.org/onto/class/google_spanner_instance"/>
    <rdfs:range rdf:resource="http://www.w3.org/2001/XMLSchema#string"/>
  </owl:DatatypeProperty>
  <owl:DatatypeProperty rdf:about="http://example.org/onto/prop/google_spanner_instance_processing_units">
    <rdfs:label>processing_units</rdfs:label>
    <rdfs:comment>The number of processing units allocated to this instance. Exactly one of either num_nodes,
processing_units or autoscaling_config must be present in terraform except when instance_type = FREE_INSTANCE.</rdfs:comment>
    <rdfs:domain rdf:resource="http://example.org/onto/class/google_spanner_instance"/>
    <rdfs:range rdf:resource="http://www.w3.org/2001/XMLSchema#string"/>
  </owl:DatatypeProperty>
  <owl:DatatypeProperty rdf:about="http://example.org/onto/prop/google_spanner_instance_project">
    <rdfs:label>project</rdfs:label>
    <rdfs:domain rdf:resource="http://example.org/onto/class/google_spanner_instance"/>
    <rdfs:range rdf:resource="http://www.w3.org/2001/XMLSchema#string"/>
  </owl:DatatypeProperty>
  <owl:DatatypeProperty rdf:about="http://example.org/onto/prop/google_spanner_instance_state">
    <rdfs:label>state</rdfs:label>
    <rdfs:comment>Instance status: 'CREATING' or 'READY'.</rdfs:comment>
    <rdfs:domain rdf:resource="http://example.org/onto/class/google_spanner_instance"/>
    <rdfs:range rdf:resource="http://www.w3.org/2001/XMLSchema#string"/>
  </owl:DatatypeProperty>
  <owl:DatatypeProperty rdf:about="http://example.org/onto/prop/google_spanner_instance_terraform_labels">
    <rdfs:label>terraform_labels</rdfs:label>
    <rdfs:comment>The combination of labels configured directly on the resource
 and default labels configured on the provider.</rdfs:comment>
    <rdfs:domain rdf:resource="http://example.org/onto/class/google_spanner_instance"/>
    <rdfs:range rdf:resource="http://www.w3.org/2001/XMLSchema#string"/>
  </owl:DatatypeProperty>
  <owl:DatatypeProperty rdf:about="http://example.org/onto/prop/google_spanner_instance_max_nodes">
    <rdfs:label>max_nodes</rdfs:label>
    <rdfs:comment>The maximum number of nodes for this specific replica.</rdfs:comment>
    <rdfs:domain rdf:resource="http://example.org/onto/class/google_spanner_instance"/>
    <rdfs:range rdf:resource="http://www.w3.org/2001/XMLSchema#string"/>
  </owl:DatatypeProperty>
  <owl:DatatypeProperty rdf:about="http://example.org/onto/prop/google_spanner_instance_min_nodes">
    <rdfs:label>min_nodes</rdfs:label>
    <rdfs:comment>The minimum number of nodes for this specific replica.</rdfs:comment>
    <rdfs:domain rdf:resource="http://example.org/onto/class/google_spanner_instance"/>
    <rdfs:range rdf:resource="http://www.w3.org/2001/XMLSchema#string"/>
  </owl:DatatypeProperty>
  <owl:DatatypeProperty rdf:about="http://example.org/onto/prop/google_spanner_instance_location">
    <rdfs:label>location</rdfs:label>
    <rdfs:comment>The location of the replica to apply asymmetric autoscaling options.</rdfs:comment>
    <rdfs:domain rdf:resource="http://example.org/onto/class/google_spanner_instance"/>
    <rdfs:range rdf:resource="http://www.w3.org/2001/XMLSchema#string"/>
  </owl:DatatypeProperty>
  <owl:DatatypeProperty rdf:about="http://example.org/onto/prop/google_spanner_instance_max_nodes">
    <rdfs:label>max_nodes</rdfs:label>
    <rdfs:comment>Specifies maximum number of nodes allocated to the instance. If set, this number
should be greater than or equal to min_nodes.</rdfs:comment>
    <rdfs:domain rdf:resource="http://example.org/onto/class/google_spanner_instance"/>
    <rdfs:range rdf:resource="http://www.w3.org/2001/XMLSchema#string"/>
  </owl:DatatypeProperty>
  <owl:DatatypeProperty rdf:about="http://example.org/onto/prop/google_spanner_instance_max_processing_units">
    <rdfs:label>max_processing_units</rdfs:label>
    <rdfs:comment>Specifies maximum number of processing units allocated to the instance.
If set, this number should be multiples of 1000 and be greater than or equal to
min_processing_units.</rdfs:comment>
    <rdfs:domain rdf:resource="http://example.org/onto/class/google_spanner_instance"/>
    <rdfs:range rdf:resource="http://www.w3.org/2001/XMLSchema#string"/>
  </owl:DatatypeProperty>
  <owl:DatatypeProperty rdf:about="http://example.org/onto/prop/google_spanner_instance_min_nodes">
    <rdfs:label>min_nodes</rdfs:label>
    <rdfs:comment>Specifies number of nodes allocated to the instance. If set, this number
should be greater than or equal to 1.</rdfs:comment>
    <rdfs:domain rdf:resource="http://example.org/onto/class/google_spanner_instance"/>
    <rdfs:range rdf:resource="http://www.w3.org/2001/XMLSchema#string"/>
  </owl:DatatypeProperty>
  <owl:DatatypeProperty rdf:about="http://example.org/onto/prop/google_spanner_instance_min_processing_units">
    <rdfs:label>min_processing_units</rdfs:label>
    <rdfs:comment>Specifies minimum number of processing units allocated to the instance.
If set, this number should be multiples of 1000.</rdfs:comment>
    <rdfs:domain rdf:resource="http://example.org/onto/class/google_spanner_instance"/>
    <rdfs:range rdf:resource="http://www.w3.org/2001/XMLSchema#string"/>
  </owl:DatatypeProperty>
  <owl:DatatypeProperty rdf:about="http://example.org/onto/prop/google_spanner_instance_high_priority_cpu_utilization_percent">
    <rdfs:label>high_priority_cpu_utilization_percent</rdfs:label>
    <rdfs:comment>Specifies the target high priority cpu utilization percentage that the autoscaler
should be trying to achieve for the instance.
This number is on a scale from 0 (no utilization) to 100 (full utilization)..</rdfs:comment>
    <rdfs:domain rdf:resource="http://example.org/onto/class/google_spanner_instance"/>
    <rdfs:range rdf:resource="http://www.w3.org/2001/XMLSchema#string"/>
  </owl:DatatypeProperty>
  <owl:DatatypeProperty rdf:about="http://example.org/onto/prop/google_spanner_instance_storage_utilization_percent">
    <rdfs:label>storage_utilization_percent</rdfs:label>
    <rdfs:comment>Specifies the target storage utilization percentage that the autoscaler
should be trying to achieve for the instance.
This number is on a scale from 0 (no utilization) to 100 (full utilization).</rdfs:comment>
    <rdfs:domain rdf:resource="http://example.org/onto/class/google_spanner_instance"/>
    <rdfs:range rdf:resource="http://www.w3.org/2001/XMLSchema#string"/>
  </owl:DatatypeProperty>
  <owl:DatatypeProperty rdf:about="http://example.org/onto/prop/google_spanner_instance_create">
    <rdfs:label>create</rdfs:label>
    <rdfs:domain rdf:resource="http://example.org/onto/class/google_spanner_instance"/>
    <rdfs:range rdf:resource="http://www.w3.org/2001/XMLSchema#string"/>
  </owl:DatatypeProperty>
  <owl:DatatypeProperty rdf:about="http://example.org/onto/prop/google_spanner_instance_delete">
    <rdfs:label>delete</rdfs:label>
    <rdfs:domain rdf:resource="http://example.org/onto/class/google_spanner_instance"/>
    <rdfs:range rdf:resource="http://www.w3.org/2001/XMLSchema#string"/>
  </owl:DatatypeProperty>
  <owl:DatatypeProperty rdf:about="http://example.org/onto/prop/google_spanner_instance_update">
    <rdfs:label>update</rdfs:label>
    <rdfs:domain rdf:resource="http://example.org/onto/class/google_spanner_instance"/>
    <rdfs:range rdf:resource="http://www.w3.org/2001/XMLSchema#string"/>
  </owl:DatatypeProperty>
</rdf:RDF>
