<?xml version="1.0" encoding="UTF-8"?>
<rdf:RDF
  xmlns:rdf="http://www.w3.org/1999/02/22-rdf-syntax-ns#"
  xmlns:rdfs="http://www.w3.org/2000/01/rdf-schema#"
  xmlns:owl="http://www.w3.org/2002/07/owl#"
  xmlns:xsd="http://www.w3.org/2001/XMLSchema#"
  xml:base="http://example.org/onto/">
  <owl:Class rdf:about="http://example.org/onto/class/google_compute_resource_policy">
    <rdfs:label>google_compute_resource_policy</rdfs:label>
    <rdfs:comment>#
#     ***     AUTO GENERATED CODE    ***    Type: MMv1     ***
#
# ----------------------------------------------------------------------------
#
#     This code is generated by Magic Modules using the following:
#
#     Configuration: https:#github.com/GoogleCloudPlatform/magic-modules/tree/main/mmv1/products/compute/ResourcePolicy.yaml
#     Template:      https:#github.com/GoogleCloudPlatform/magic-modules/tree/main/mmv1/templates/terraform/resource.html.markdown.tmpl
#
#     DO NOT EDIT this file directly. Any changes made to this file will be
#     overwritten during the next generation cycle.
#
# ----------------------------------------------------------------------------
subcategory: "Compute Engine"
description: |-
  A policy that can be attached to a resource to specify or schedule actions on that resource.
---</rdfs:comment>
  </owl:Class>
  <owl:DatatypeProperty rdf:about="http://example.org/onto/prop/google_compute_resource_policy_description">
    <rdfs:label>description</rdfs:label>
    <rdfs:comment>An optional description of this resource. Provide this property when you create the resource.</rdfs:comment>
    <rdfs:domain rdf:resource="http://example.org/onto/class/google_compute_resource_policy"/>
    <rdfs:range rdf:resource="http://www.w3.org/2001/XMLSchema#string"/>
  </owl:DatatypeProperty>
  <owl:DatatypeProperty rdf:about="http://example.org/onto/prop/google_compute_resource_policy_id">
    <rdfs:label>id</rdfs:label>
    <rdfs:domain rdf:resource="http://example.org/onto/class/google_compute_resource_policy"/>
    <rdfs:range rdf:resource="http://www.w3.org/2001/XMLSchema#string"/>
  </owl:DatatypeProperty>
  <owl:DatatypeProperty rdf:about="http://example.org/onto/prop/google_compute_resource_policy_name">
    <rdfs:label>name</rdfs:label>
    <rdfs:comment>The name of the resource, provided by the client when initially creating
the resource. The resource name must be 1-63 characters long, and comply
with RFC1035. Specifically, the name must be 1-63 characters long and
match the regular expression '[a-z]([-a-z0-9]*[a-z0-9])'? which means the
first character must be a lowercase letter, and all following characters
must be a dash, lowercase letter, or digit, except the last character,
which cannot be a dash.</rdfs:comment>
    <rdfs:domain rdf:resource="http://example.org/onto/class/google_compute_resource_policy"/>
    <rdfs:range rdf:resource="http://www.w3.org/2001/XMLSchema#string"/>
  </owl:DatatypeProperty>
  <owl:DatatypeProperty rdf:about="http://example.org/onto/prop/google_compute_resource_policy_project">
    <rdfs:label>project</rdfs:label>
    <rdfs:domain rdf:resource="http://example.org/onto/class/google_compute_resource_policy"/>
    <rdfs:range rdf:resource="http://www.w3.org/2001/XMLSchema#string"/>
  </owl:DatatypeProperty>
  <owl:DatatypeProperty rdf:about="http://example.org/onto/prop/google_compute_resource_policy_region">
    <rdfs:label>region</rdfs:label>
    <rdfs:comment>Region where resource policy resides.</rdfs:comment>
    <rdfs:domain rdf:resource="http://example.org/onto/class/google_compute_resource_policy"/>
    <rdfs:range rdf:resource="http://www.w3.org/2001/XMLSchema#string"/>
  </owl:DatatypeProperty>
  <owl:DatatypeProperty rdf:about="http://example.org/onto/prop/google_compute_resource_policy_self_link">
    <rdfs:label>self_link</rdfs:label>
    <rdfs:domain rdf:resource="http://example.org/onto/class/google_compute_resource_policy"/>
    <rdfs:range rdf:resource="http://www.w3.org/2001/XMLSchema#string"/>
  </owl:DatatypeProperty>
  <owl:DatatypeProperty rdf:about="http://example.org/onto/prop/google_compute_resource_policy_enabled">
    <rdfs:label>enabled</rdfs:label>
    <rdfs:comment>Enable disk consistency on the resource policy.</rdfs:comment>
    <rdfs:domain rdf:resource="http://example.org/onto/class/google_compute_resource_policy"/>
    <rdfs:range rdf:resource="http://www.w3.org/2001/XMLSchema#string"/>
  </owl:DatatypeProperty>
  <owl:DatatypeProperty rdf:about="http://example.org/onto/prop/google_compute_resource_policy_availability_domain_count">
    <rdfs:label>availability_domain_count</rdfs:label>
    <rdfs:comment>The number of availability domains instances will be spread across. If two instances are in different
availability domain, they will not be put in the same low latency network</rdfs:comment>
    <rdfs:domain rdf:resource="http://example.org/onto/class/google_compute_resource_policy"/>
    <rdfs:range rdf:resource="http://www.w3.org/2001/XMLSchema#string"/>
  </owl:DatatypeProperty>
  <owl:DatatypeProperty rdf:about="http://example.org/onto/prop/google_compute_resource_policy_collocation">
    <rdfs:label>collocation</rdfs:label>
    <rdfs:comment>Collocation specifies whether to place VMs inside the same availability domain on the same low-latency network.
Specify 'COLLOCATED' to enable collocation. Can only be specified with 'vm_count'. If compute instances are created
with a COLLOCATED policy, then exactly 'vm_count' instances must be created at the same time with the resource policy
attached. Possible values: ["COLLOCATED"]</rdfs:comment>
    <rdfs:domain rdf:resource="http://example.org/onto/class/google_compute_resource_policy"/>
    <rdfs:range rdf:resource="http://www.w3.org/2001/XMLSchema#string"/>
  </owl:DatatypeProperty>
  <owl:DatatypeProperty rdf:about="http://example.org/onto/prop/google_compute_resource_policy_gpu_topology">
    <rdfs:label>gpu_topology</rdfs:label>
    <rdfs:comment>Specifies the shape of the GPU slice, in slice based GPU families eg. A4X.</rdfs:comment>
    <rdfs:domain rdf:resource="http://example.org/onto/class/google_compute_resource_policy"/>
    <rdfs:range rdf:resource="http://www.w3.org/2001/XMLSchema#string"/>
  </owl:DatatypeProperty>
  <owl:DatatypeProperty rdf:about="http://example.org/onto/prop/google_compute_resource_policy_vm_count">
    <rdfs:label>vm_count</rdfs:label>
    <rdfs:comment>Number of VMs in this placement group. Google does not recommend that you use this field
unless you use a compact policy and you want your policy to work only if it contains this
exact number of VMs.</rdfs:comment>
    <rdfs:domain rdf:resource="http://example.org/onto/class/google_compute_resource_policy"/>
    <rdfs:range rdf:resource="http://www.w3.org/2001/XMLSchema#string"/>
  </owl:DatatypeProperty>
  <owl:DatatypeProperty rdf:about="http://example.org/onto/prop/google_compute_resource_policy_expiration_time">
    <rdfs:label>expiration_time</rdfs:label>
    <rdfs:comment>The expiration time of the schedule. The timestamp is an RFC3339 string.</rdfs:comment>
    <rdfs:domain rdf:resource="http://example.org/onto/class/google_compute_resource_policy"/>
    <rdfs:range rdf:resource="http://www.w3.org/2001/XMLSchema#string"/>
  </owl:DatatypeProperty>
  <owl:DatatypeProperty rdf:about="http://example.org/onto/prop/google_compute_resource_policy_start_time">
    <rdfs:label>start_time</rdfs:label>
    <rdfs:comment>The start time of the schedule. The timestamp is an RFC3339 string.</rdfs:comment>
    <rdfs:domain rdf:resource="http://example.org/onto/class/google_compute_resource_policy"/>
    <rdfs:range rdf:resource="http://www.w3.org/2001/XMLSchema#string"/>
  </owl:DatatypeProperty>
  <owl:DatatypeProperty rdf:about="http://example.org/onto/prop/google_compute_resource_policy_time_zone">
    <rdfs:label>time_zone</rdfs:label>
    <rdfs:comment>Specifies the time zone to be used in interpreting the schedule. The value of this field must be a time zone name
from the tz database: http://en.wikipedia.org/wiki/Tz_database.</rdfs:comment>
    <rdfs:domain rdf:resource="http://example.org/onto/class/google_compute_resource_policy"/>
    <rdfs:range rdf:resource="http://www.w3.org/2001/XMLSchema#string"/>
  </owl:DatatypeProperty>
  <owl:DatatypeProperty rdf:about="http://example.org/onto/prop/google_compute_resource_policy_schedule">
    <rdfs:label>schedule</rdfs:label>
    <rdfs:comment>Specifies the frequency for the operation, using the unix-cron format.</rdfs:comment>
    <rdfs:domain rdf:resource="http://example.org/onto/class/google_compute_resource_policy"/>
    <rdfs:range rdf:resource="http://www.w3.org/2001/XMLSchema#string"/>
  </owl:DatatypeProperty>
  <owl:DatatypeProperty rdf:about="http://example.org/onto/prop/google_compute_resource_policy_schedule">
    <rdfs:label>schedule</rdfs:label>
    <rdfs:comment>Specifies the frequency for the operation, using the unix-cron format.</rdfs:comment>
    <rdfs:domain rdf:resource="http://example.org/onto/class/google_compute_resource_policy"/>
    <rdfs:range rdf:resource="http://www.w3.org/2001/XMLSchema#string"/>
  </owl:DatatypeProperty>
  <owl:DatatypeProperty rdf:about="http://example.org/onto/prop/google_compute_resource_policy_max_retention_days">
    <rdfs:label>max_retention_days</rdfs:label>
    <rdfs:comment>Maximum age of the snapshot that is allowed to be kept.</rdfs:comment>
    <rdfs:domain rdf:resource="http://example.org/onto/class/google_compute_resource_policy"/>
    <rdfs:range rdf:resource="http://www.w3.org/2001/XMLSchema#string"/>
  </owl:DatatypeProperty>
  <owl:DatatypeProperty rdf:about="http://example.org/onto/prop/google_compute_resource_policy_on_source_disk_delete">
    <rdfs:label>on_source_disk_delete</rdfs:label>
    <rdfs:comment>Specifies the behavior to apply to scheduled snapshots when
the source disk is deleted. Default value: "KEEP_AUTO_SNAPSHOTS" Possible values: ["KEEP_AUTO_SNAPSHOTS", "APPLY_RETENTION_POLICY"]</rdfs:comment>
    <rdfs:domain rdf:resource="http://example.org/onto/class/google_compute_resource_policy"/>
    <rdfs:range rdf:resource="http://www.w3.org/2001/XMLSchema#string"/>
  </owl:DatatypeProperty>
  <owl:DatatypeProperty rdf:about="http://example.org/onto/prop/google_compute_resource_policy_days_in_cycle">
    <rdfs:label>days_in_cycle</rdfs:label>
    <rdfs:comment>Defines a schedule with units measured in days. The value determines how many days pass between the start of each cycle. Days in cycle for snapshot schedule policy must be 1.</rdfs:comment>
    <rdfs:domain rdf:resource="http://example.org/onto/class/google_compute_resource_policy"/>
    <rdfs:range rdf:resource="http://www.w3.org/2001/XMLSchema#string"/>
  </owl:DatatypeProperty>
  <owl:DatatypeProperty rdf:about="http://example.org/onto/prop/google_compute_resource_policy_start_time">
    <rdfs:label>start_time</rdfs:label>
    <rdfs:comment>This must be in UTC format that resolves to one of
00:00, 04:00, 08:00, 12:00, 16:00, or 20:00. For example,
both 13:00-5 and 08:00 are valid.</rdfs:comment>
    <rdfs:domain rdf:resource="http://example.org/onto/class/google_compute_resource_policy"/>
    <rdfs:range rdf:resource="http://www.w3.org/2001/XMLSchema#string"/>
  </owl:DatatypeProperty>
  <owl:DatatypeProperty rdf:about="http://example.org/onto/prop/google_compute_resource_policy_hours_in_cycle">
    <rdfs:label>hours_in_cycle</rdfs:label>
    <rdfs:comment>The number of hours between snapshots.</rdfs:comment>
    <rdfs:domain rdf:resource="http://example.org/onto/class/google_compute_resource_policy"/>
    <rdfs:range rdf:resource="http://www.w3.org/2001/XMLSchema#string"/>
  </owl:DatatypeProperty>
  <owl:DatatypeProperty rdf:about="http://example.org/onto/prop/google_compute_resource_policy_start_time">
    <rdfs:label>start_time</rdfs:label>
    <rdfs:comment>Time within the window to start the operations.
It must be in an hourly format "HH:MM",
where HH : [00-23] and MM : [00] GMT. eg: 21:00</rdfs:comment>
    <rdfs:domain rdf:resource="http://example.org/onto/class/google_compute_resource_policy"/>
    <rdfs:range rdf:resource="http://www.w3.org/2001/XMLSchema#string"/>
  </owl:DatatypeProperty>
  <owl:DatatypeProperty rdf:about="http://example.org/onto/prop/google_compute_resource_policy_day">
    <rdfs:label>day</rdfs:label>
    <rdfs:comment>The day of the week to create the snapshot. e.g. MONDAY Possible values: ["MONDAY", "TUESDAY", "WEDNESDAY", "THURSDAY", "FRIDAY", "SATURDAY", "SUNDAY"]</rdfs:comment>
    <rdfs:domain rdf:resource="http://example.org/onto/class/google_compute_resource_policy"/>
    <rdfs:range rdf:resource="http://www.w3.org/2001/XMLSchema#string"/>
  </owl:DatatypeProperty>
  <owl:DatatypeProperty rdf:about="http://example.org/onto/prop/google_compute_resource_policy_start_time">
    <rdfs:label>start_time</rdfs:label>
    <rdfs:comment>Time within the window to start the operations.
It must be in format "HH:MM", where HH : [00-23] and MM : [00-00] GMT.</rdfs:comment>
    <rdfs:domain rdf:resource="http://example.org/onto/class/google_compute_resource_policy"/>
    <rdfs:range rdf:resource="http://www.w3.org/2001/XMLSchema#string"/>
  </owl:DatatypeProperty>
  <owl:DatatypeProperty rdf:about="http://example.org/onto/prop/google_compute_resource_policy_chain_name">
    <rdfs:label>chain_name</rdfs:label>
    <rdfs:comment>Creates the new snapshot in the snapshot chain labeled with the
specified name. The chain name must be 1-63 characters long and comply
with RFC1035.</rdfs:comment>
    <rdfs:domain rdf:resource="http://example.org/onto/class/google_compute_resource_policy"/>
    <rdfs:range rdf:resource="http://www.w3.org/2001/XMLSchema#string"/>
  </owl:DatatypeProperty>
  <owl:DatatypeProperty rdf:about="http://example.org/onto/prop/google_compute_resource_policy_guest_flush">
    <rdfs:label>guest_flush</rdfs:label>
    <rdfs:comment>Whether to perform a 'guest aware' snapshot.</rdfs:comment>
    <rdfs:domain rdf:resource="http://example.org/onto/class/google_compute_resource_policy"/>
    <rdfs:range rdf:resource="http://www.w3.org/2001/XMLSchema#string"/>
  </owl:DatatypeProperty>
  <owl:DatatypeProperty rdf:about="http://example.org/onto/prop/google_compute_resource_policy_labels">
    <rdfs:label>labels</rdfs:label>
    <rdfs:comment>A set of key-value pairs.</rdfs:comment>
    <rdfs:domain rdf:resource="http://example.org/onto/class/google_compute_resource_policy"/>
    <rdfs:range rdf:resource="http://www.w3.org/2001/XMLSchema#string"/>
  </owl:DatatypeProperty>
  <owl:DatatypeProperty rdf:about="http://example.org/onto/prop/google_compute_resource_policy_storage_locations">
    <rdfs:label>storage_locations</rdfs:label>
    <rdfs:comment>Cloud Storage bucket location to store the auto snapshot
(regional or multi-regional)</rdfs:comment>
    <rdfs:domain rdf:resource="http://example.org/onto/class/google_compute_resource_policy"/>
    <rdfs:range rdf:resource="http://www.w3.org/2001/XMLSchema#string"/>
  </owl:DatatypeProperty>
  <owl:DatatypeProperty rdf:about="http://example.org/onto/prop/google_compute_resource_policy_create">
    <rdfs:label>create</rdfs:label>
    <rdfs:domain rdf:resource="http://example.org/onto/class/google_compute_resource_policy"/>
    <rdfs:range rdf:resource="http://www.w3.org/2001/XMLSchema#string"/>
  </owl:DatatypeProperty>
  <owl:DatatypeProperty rdf:about="http://example.org/onto/prop/google_compute_resource_policy_delete">
    <rdfs:label>delete</rdfs:label>
    <rdfs:domain rdf:resource="http://example.org/onto/class/google_compute_resource_policy"/>
    <rdfs:range rdf:resource="http://www.w3.org/2001/XMLSchema#string"/>
  </owl:DatatypeProperty>
  <owl:DatatypeProperty rdf:about="http://example.org/onto/prop/google_compute_resource_policy_update">
    <rdfs:label>update</rdfs:label>
    <rdfs:domain rdf:resource="http://example.org/onto/class/google_compute_resource_policy"/>
    <rdfs:range rdf:resource="http://www.w3.org/2001/XMLSchema#string"/>
  </owl:DatatypeProperty>
  <owl:DatatypeProperty rdf:about="http://example.org/onto/prop/google_compute_resource_policy_accelerator_topology">
    <rdfs:label>accelerator_topology</rdfs:label>
    <rdfs:comment>The accelerator topology. This field can be set only when the workload policy type is HIGH_THROUGHPUT
and cannot be set if max topology distance is set.</rdfs:comment>
    <rdfs:domain rdf:resource="http://example.org/onto/class/google_compute_resource_policy"/>
    <rdfs:range rdf:resource="http://www.w3.org/2001/XMLSchema#string"/>
  </owl:DatatypeProperty>
  <owl:DatatypeProperty rdf:about="http://example.org/onto/prop/google_compute_resource_policy_max_topology_distance">
    <rdfs:label>max_topology_distance</rdfs:label>
    <rdfs:comment>The maximum topology distance. This field can be set only when the workload policy type is HIGH_THROUGHPUT
and cannot be set if accelerator topology is set. Possible values: ["BLOCK", "CLUSTER", "SUBBLOCK"]</rdfs:comment>
    <rdfs:domain rdf:resource="http://example.org/onto/class/google_compute_resource_policy"/>
    <rdfs:range rdf:resource="http://www.w3.org/2001/XMLSchema#string"/>
  </owl:DatatypeProperty>
  <owl:DatatypeProperty rdf:about="http://example.org/onto/prop/google_compute_resource_policy_type">
    <rdfs:label>type</rdfs:label>
    <rdfs:comment>The type of workload policy. Possible values: ["HIGH_AVAILABILITY", "HIGH_THROUGHPUT"]</rdfs:comment>
    <rdfs:domain rdf:resource="http://example.org/onto/class/google_compute_resource_policy"/>
    <rdfs:range rdf:resource="http://www.w3.org/2001/XMLSchema#string"/>
  </owl:DatatypeProperty>
</rdf:RDF>
