<?xml version="1.0" encoding="UTF-8"?>
<rdf:RDF
  xmlns:rdf="http://www.w3.org/1999/02/22-rdf-syntax-ns#"
  xmlns:rdfs="http://www.w3.org/2000/01/rdf-schema#"
  xmlns:owl="http://www.w3.org/2002/07/owl#"
  xmlns:xsd="http://www.w3.org/2001/XMLSchema#"
  xml:base="http://example.org/onto/">
  <owl:Class rdf:about="http://example.org/onto/class/google_integrations_client">
    <rdfs:label>google_integrations_client</rdfs:label>
    <rdfs:comment>#
#     ***     AUTO GENERATED CODE    ***    Type: MMv1     ***
#
# ----------------------------------------------------------------------------
#
#     This code is generated by Magic Modules using the following:
#
#     Configuration: https:#github.com/GoogleCloudPlatform/magic-modules/tree/main/mmv1/products/integrations/Client.yaml
#     Template:      https:#github.com/GoogleCloudPlatform/magic-modules/tree/main/mmv1/templates/terraform/resource.html.markdown.tmpl
#
#     DO NOT EDIT this file directly. Any changes made to this file will be
#     overwritten during the next generation cycle.
#
# ----------------------------------------------------------------------------
subcategory: "Application Integration"
description: |-
  Application Integration Client.
---</rdfs:comment>
  </owl:Class>
  <owl:DatatypeProperty rdf:about="http://example.org/onto/prop/google_integrations_client_create_sample_integrations">
    <rdfs:label>create_sample_integrations</rdfs:label>
    <rdfs:comment>Indicates if sample integrations should be created along with provisioning.</rdfs:comment>
    <rdfs:domain rdf:resource="http://example.org/onto/class/google_integrations_client"/>
    <rdfs:range rdf:resource="http://www.w3.org/2001/XMLSchema#string"/>
  </owl:DatatypeProperty>
  <owl:DatatypeProperty rdf:about="http://example.org/onto/prop/google_integrations_client_id">
    <rdfs:label>id</rdfs:label>
    <rdfs:domain rdf:resource="http://example.org/onto/class/google_integrations_client"/>
    <rdfs:range rdf:resource="http://www.w3.org/2001/XMLSchema#string"/>
  </owl:DatatypeProperty>
  <owl:DatatypeProperty rdf:about="http://example.org/onto/prop/google_integrations_client_location">
    <rdfs:label>location</rdfs:label>
    <rdfs:comment>Location in which client needs to be provisioned.</rdfs:comment>
    <rdfs:domain rdf:resource="http://example.org/onto/class/google_integrations_client"/>
    <rdfs:range rdf:resource="http://www.w3.org/2001/XMLSchema#string"/>
  </owl:DatatypeProperty>
  <owl:DatatypeProperty rdf:about="http://example.org/onto/prop/google_integrations_client_project">
    <rdfs:label>project</rdfs:label>
    <rdfs:domain rdf:resource="http://example.org/onto/class/google_integrations_client"/>
    <rdfs:range rdf:resource="http://www.w3.org/2001/XMLSchema#string"/>
  </owl:DatatypeProperty>
  <owl:DatatypeProperty rdf:about="http://example.org/onto/prop/google_integrations_client_run_as_service_account">
    <rdfs:label>run_as_service_account</rdfs:label>
    <rdfs:comment>User input run-as service account, if empty, will bring up a new default service account.</rdfs:comment>
    <rdfs:domain rdf:resource="http://example.org/onto/class/google_integrations_client"/>
    <rdfs:range rdf:resource="http://www.w3.org/2001/XMLSchema#string"/>
  </owl:DatatypeProperty>
  <owl:DatatypeProperty rdf:about="http://example.org/onto/prop/google_integrations_client_key">
    <rdfs:label>key</rdfs:label>
    <rdfs:comment>A Cloud KMS key is a named object containing one or more key versions, along
with metadata for the key. A key exists on exactly one key ring tied to a
specific location.</rdfs:comment>
    <rdfs:domain rdf:resource="http://example.org/onto/class/google_integrations_client"/>
    <rdfs:range rdf:resource="http://www.w3.org/2001/XMLSchema#string"/>
  </owl:DatatypeProperty>
  <owl:DatatypeProperty rdf:about="http://example.org/onto/prop/google_integrations_client_key_version">
    <rdfs:label>key_version</rdfs:label>
    <rdfs:comment>Each version of a key contains key material used for encryption or signing.
A key's version is represented by an integer, starting at 1. To decrypt data
or verify a signature, you must use the same key version that was used to
encrypt or sign the data.</rdfs:comment>
    <rdfs:domain rdf:resource="http://example.org/onto/class/google_integrations_client"/>
    <rdfs:range rdf:resource="http://www.w3.org/2001/XMLSchema#string"/>
  </owl:DatatypeProperty>
  <owl:DatatypeProperty rdf:about="http://example.org/onto/prop/google_integrations_client_kms_location">
    <rdfs:label>kms_location</rdfs:label>
    <rdfs:comment>Location name of the key ring, e.g. "us-west1".</rdfs:comment>
    <rdfs:domain rdf:resource="http://example.org/onto/class/google_integrations_client"/>
    <rdfs:range rdf:resource="http://www.w3.org/2001/XMLSchema#string"/>
  </owl:DatatypeProperty>
  <owl:DatatypeProperty rdf:about="http://example.org/onto/prop/google_integrations_client_kms_project_id">
    <rdfs:label>kms_project_id</rdfs:label>
    <rdfs:comment>The Google Cloud project id of the project where the kms key stored. If empty,
the kms key is stored at the same project as customer's project and ecrypted
with CMEK, otherwise, the kms key is stored in the tenant project and
encrypted with GMEK.</rdfs:comment>
    <rdfs:domain rdf:resource="http://example.org/onto/class/google_integrations_client"/>
    <rdfs:range rdf:resource="http://www.w3.org/2001/XMLSchema#string"/>
  </owl:DatatypeProperty>
  <owl:DatatypeProperty rdf:about="http://example.org/onto/prop/google_integrations_client_kms_ring">
    <rdfs:label>kms_ring</rdfs:label>
    <rdfs:comment>A key ring organizes keys in a specific Google Cloud location and allows you to
manage access control on groups of keys. A key ring's name does not need to be
unique across a Google Cloud project, but must be unique within a given location.</rdfs:comment>
    <rdfs:domain rdf:resource="http://example.org/onto/class/google_integrations_client"/>
    <rdfs:range rdf:resource="http://www.w3.org/2001/XMLSchema#string"/>
  </owl:DatatypeProperty>
  <owl:DatatypeProperty rdf:about="http://example.org/onto/prop/google_integrations_client_create">
    <rdfs:label>create</rdfs:label>
    <rdfs:domain rdf:resource="http://example.org/onto/class/google_integrations_client"/>
    <rdfs:range rdf:resource="http://www.w3.org/2001/XMLSchema#string"/>
  </owl:DatatypeProperty>
  <owl:DatatypeProperty rdf:about="http://example.org/onto/prop/google_integrations_client_delete">
    <rdfs:label>delete</rdfs:label>
    <rdfs:domain rdf:resource="http://example.org/onto/class/google_integrations_client"/>
    <rdfs:range rdf:resource="http://www.w3.org/2001/XMLSchema#string"/>
  </owl:DatatypeProperty>
</rdf:RDF>
