<?xml version="1.0" encoding="UTF-8"?>
<rdf:RDF
  xmlns:rdf="http://www.w3.org/1999/02/22-rdf-syntax-ns#"
  xmlns:rdfs="http://www.w3.org/2000/01/rdf-schema#"
  xmlns:owl="http://www.w3.org/2002/07/owl#"
  xmlns:xsd="http://www.w3.org/2001/XMLSchema#"
  xml:base="http://example.org/onto/">
  <owl:Class rdf:about="http://example.org/onto/class/google_iam_oauth_client_credential">
    <rdfs:label>google_iam_oauth_client_credential</rdfs:label>
    <rdfs:comment>#
#     ***     AUTO GENERATED CODE    ***    Type: MMv1     ***
#
# ----------------------------------------------------------------------------
#
#     This code is generated by Magic Modules using the following:
#
#     Configuration: https:#github.com/GoogleCloudPlatform/magic-modules/tree/main/mmv1/products/iamworkforcepool/OauthClientCredential.yaml
#     Template:      https:#github.com/GoogleCloudPlatform/magic-modules/tree/main/mmv1/templates/terraform/resource.html.markdown.tmpl
#
#     DO NOT EDIT this file directly. Any changes made to this file will be
#     overwritten during the next generation cycle.
#
# ----------------------------------------------------------------------------
subcategory: "Cloud IAM"
description: |-
  Represents an OAuth Client Credential.
---</rdfs:comment>
  </owl:Class>
  <owl:DatatypeProperty rdf:about="http://example.org/onto/prop/google_iam_oauth_client_credential_client_secret">
    <rdfs:label>client_secret</rdfs:label>
    <rdfs:comment>The system-generated OAuth client secret.

The client secret must be stored securely. If the client secret is
leaked, you must delete and re-create the client credential. To learn
more, see [OAuth client and credential security risks and
mitigations](https://cloud.google.com/iam/docs/workforce-oauth-app#security)</rdfs:comment>
    <rdfs:domain rdf:resource="http://example.org/onto/class/google_iam_oauth_client_credential"/>
    <rdfs:range rdf:resource="http://www.w3.org/2001/XMLSchema#string"/>
  </owl:DatatypeProperty>
  <owl:DatatypeProperty rdf:about="http://example.org/onto/prop/google_iam_oauth_client_credential_disabled">
    <rdfs:label>disabled</rdfs:label>
    <rdfs:comment>Whether the OauthClientCredential is disabled. You cannot use a
disabled OauthClientCredential.</rdfs:comment>
    <rdfs:domain rdf:resource="http://example.org/onto/class/google_iam_oauth_client_credential"/>
    <rdfs:range rdf:resource="http://www.w3.org/2001/XMLSchema#string"/>
  </owl:DatatypeProperty>
  <owl:DatatypeProperty rdf:about="http://example.org/onto/prop/google_iam_oauth_client_credential_display_name">
    <rdfs:label>display_name</rdfs:label>
    <rdfs:comment>A user-specified display name of the OauthClientCredential.

Cannot exceed 32 characters.</rdfs:comment>
    <rdfs:domain rdf:resource="http://example.org/onto/class/google_iam_oauth_client_credential"/>
    <rdfs:range rdf:resource="http://www.w3.org/2001/XMLSchema#string"/>
  </owl:DatatypeProperty>
  <owl:DatatypeProperty rdf:about="http://example.org/onto/prop/google_iam_oauth_client_credential_id">
    <rdfs:label>id</rdfs:label>
    <rdfs:domain rdf:resource="http://example.org/onto/class/google_iam_oauth_client_credential"/>
    <rdfs:range rdf:resource="http://www.w3.org/2001/XMLSchema#string"/>
  </owl:DatatypeProperty>
  <owl:DatatypeProperty rdf:about="http://example.org/onto/prop/google_iam_oauth_client_credential_location">
    <rdfs:label>location</rdfs:label>
    <rdfs:comment>Resource ID segment making up resource 'name'. It identifies the resource within its parent collection as described in https://google.aip.dev/122.</rdfs:comment>
    <rdfs:domain rdf:resource="http://example.org/onto/class/google_iam_oauth_client_credential"/>
    <rdfs:range rdf:resource="http://www.w3.org/2001/XMLSchema#string"/>
  </owl:DatatypeProperty>
  <owl:DatatypeProperty rdf:about="http://example.org/onto/prop/google_iam_oauth_client_credential_name">
    <rdfs:label>name</rdfs:label>
    <rdfs:comment>Immutable. Identifier. The resource name of the OauthClientCredential.

Format:
'projects/{project}/locations/{location}/oauthClients/{oauth_client}/credentials/{credential}'</rdfs:comment>
    <rdfs:domain rdf:resource="http://example.org/onto/class/google_iam_oauth_client_credential"/>
    <rdfs:range rdf:resource="http://www.w3.org/2001/XMLSchema#string"/>
  </owl:DatatypeProperty>
  <owl:DatatypeProperty rdf:about="http://example.org/onto/prop/google_iam_oauth_client_credential_oauth_client_credential_id">
    <rdfs:label>oauth_client_credential_id</rdfs:label>
    <rdfs:comment>Required. The ID to use for the OauthClientCredential, which becomes the
final component of the resource name. This value should be 4-32 characters,
and may contain the characters [a-z0-9-]. The prefix 'gcp-' is
reserved for use by Google, and may not be specified.</rdfs:comment>
    <rdfs:domain rdf:resource="http://example.org/onto/class/google_iam_oauth_client_credential"/>
    <rdfs:range rdf:resource="http://www.w3.org/2001/XMLSchema#string"/>
  </owl:DatatypeProperty>
  <owl:DatatypeProperty rdf:about="http://example.org/onto/prop/google_iam_oauth_client_credential_oauthclient">
    <rdfs:label>oauthclient</rdfs:label>
    <rdfs:comment>Resource ID segment making up resource 'name'. It identifies the resource within its parent collection as described in https://google.aip.dev/122.</rdfs:comment>
    <rdfs:domain rdf:resource="http://example.org/onto/class/google_iam_oauth_client_credential"/>
    <rdfs:range rdf:resource="http://www.w3.org/2001/XMLSchema#string"/>
  </owl:DatatypeProperty>
  <owl:DatatypeProperty rdf:about="http://example.org/onto/prop/google_iam_oauth_client_credential_project">
    <rdfs:label>project</rdfs:label>
    <rdfs:domain rdf:resource="http://example.org/onto/class/google_iam_oauth_client_credential"/>
    <rdfs:range rdf:resource="http://www.w3.org/2001/XMLSchema#string"/>
  </owl:DatatypeProperty>
  <owl:DatatypeProperty rdf:about="http://example.org/onto/prop/google_iam_oauth_client_credential_create">
    <rdfs:label>create</rdfs:label>
    <rdfs:domain rdf:resource="http://example.org/onto/class/google_iam_oauth_client_credential"/>
    <rdfs:range rdf:resource="http://www.w3.org/2001/XMLSchema#string"/>
  </owl:DatatypeProperty>
  <owl:DatatypeProperty rdf:about="http://example.org/onto/prop/google_iam_oauth_client_credential_delete">
    <rdfs:label>delete</rdfs:label>
    <rdfs:domain rdf:resource="http://example.org/onto/class/google_iam_oauth_client_credential"/>
    <rdfs:range rdf:resource="http://www.w3.org/2001/XMLSchema#string"/>
  </owl:DatatypeProperty>
  <owl:DatatypeProperty rdf:about="http://example.org/onto/prop/google_iam_oauth_client_credential_update">
    <rdfs:label>update</rdfs:label>
    <rdfs:domain rdf:resource="http://example.org/onto/class/google_iam_oauth_client_credential"/>
    <rdfs:range rdf:resource="http://www.w3.org/2001/XMLSchema#string"/>
  </owl:DatatypeProperty>
</rdf:RDF>
