<?xml version="1.0" encoding="UTF-8"?>
<rdf:RDF
  xmlns:rdf="http://www.w3.org/1999/02/22-rdf-syntax-ns#"
  xmlns:rdfs="http://www.w3.org/2000/01/rdf-schema#"
  xmlns:owl="http://www.w3.org/2002/07/owl#"
  xmlns:xsd="http://www.w3.org/2001/XMLSchema#"
  xml:base="http://example.org/onto/">
  <owl:Class rdf:about="http://example.org/onto/class/google_edgenetwork_interconnect_attachment">
    <rdfs:label>google_edgenetwork_interconnect_attachment</rdfs:label>
    <rdfs:comment>#
#     ***     AUTO GENERATED CODE    ***    Type: MMv1     ***
#
# ----------------------------------------------------------------------------
#
#     This code is generated by Magic Modules using the following:
#
#     Configuration: https:#github.com/GoogleCloudPlatform/magic-modules/tree/main/mmv1/products/edgenetwork/InterconnectAttachment.yaml
#     Template:      https:#github.com/GoogleCloudPlatform/magic-modules/tree/main/mmv1/templates/terraform/resource.html.markdown.tmpl
#
#     DO NOT EDIT this file directly. Any changes made to this file will be
#     overwritten during the next generation cycle.
#
# ----------------------------------------------------------------------------
subcategory: "Distributed Cloud Edge Network"
description: |-
  A Distributed Cloud Edge interconnect attachment, which connects routers to the northbound network.
---</rdfs:comment>
  </owl:Class>
  <owl:DatatypeProperty rdf:about="http://example.org/onto/prop/google_edgenetwork_interconnect_attachment_create_time">
    <rdfs:label>create_time</rdfs:label>
    <rdfs:comment>The time when the resource was created.
A timestamp in RFC3339 UTC "Zulu" format, with nanosecond resolution and up to nine
fractional digits. Examples: '2014-10-02T15:01:23Z' and '2014-10-02T15:01:23.045123456Z'.</rdfs:comment>
    <rdfs:domain rdf:resource="http://example.org/onto/class/google_edgenetwork_interconnect_attachment"/>
    <rdfs:range rdf:resource="http://www.w3.org/2001/XMLSchema#string"/>
  </owl:DatatypeProperty>
  <owl:DatatypeProperty rdf:about="http://example.org/onto/prop/google_edgenetwork_interconnect_attachment_description">
    <rdfs:label>description</rdfs:label>
    <rdfs:comment>A free-text description of the resource. Max length 1024 characters.</rdfs:comment>
    <rdfs:domain rdf:resource="http://example.org/onto/class/google_edgenetwork_interconnect_attachment"/>
    <rdfs:range rdf:resource="http://www.w3.org/2001/XMLSchema#string"/>
  </owl:DatatypeProperty>
  <owl:DatatypeProperty rdf:about="http://example.org/onto/prop/google_edgenetwork_interconnect_attachment_effective_labels">
    <rdfs:label>effective_labels</rdfs:label>
    <rdfs:comment>All of labels (key/value pairs) present on the resource in GCP, including the labels configured through Terraform, other clients and services.</rdfs:comment>
    <rdfs:domain rdf:resource="http://example.org/onto/class/google_edgenetwork_interconnect_attachment"/>
    <rdfs:range rdf:resource="http://www.w3.org/2001/XMLSchema#string"/>
  </owl:DatatypeProperty>
  <owl:DatatypeProperty rdf:about="http://example.org/onto/prop/google_edgenetwork_interconnect_attachment_id">
    <rdfs:label>id</rdfs:label>
    <rdfs:domain rdf:resource="http://example.org/onto/class/google_edgenetwork_interconnect_attachment"/>
    <rdfs:range rdf:resource="http://www.w3.org/2001/XMLSchema#string"/>
  </owl:DatatypeProperty>
  <owl:DatatypeProperty rdf:about="http://example.org/onto/prop/google_edgenetwork_interconnect_attachment_interconnect">
    <rdfs:label>interconnect</rdfs:label>
    <rdfs:comment>The ID of the underlying interconnect that this attachment's traffic will traverse through.</rdfs:comment>
    <rdfs:domain rdf:resource="http://example.org/onto/class/google_edgenetwork_interconnect_attachment"/>
    <rdfs:range rdf:resource="http://www.w3.org/2001/XMLSchema#string"/>
  </owl:DatatypeProperty>
  <owl:DatatypeProperty rdf:about="http://example.org/onto/prop/google_edgenetwork_interconnect_attachment_interconnect_attachment_id">
    <rdfs:label>interconnect_attachment_id</rdfs:label>
    <rdfs:comment>A unique ID that identifies this interconnect attachment.</rdfs:comment>
    <rdfs:domain rdf:resource="http://example.org/onto/class/google_edgenetwork_interconnect_attachment"/>
    <rdfs:range rdf:resource="http://www.w3.org/2001/XMLSchema#string"/>
  </owl:DatatypeProperty>
  <owl:DatatypeProperty rdf:about="http://example.org/onto/prop/google_edgenetwork_interconnect_attachment_labels">
    <rdfs:label>labels</rdfs:label>
    <rdfs:comment>Labels associated with this resource.


**Note**: This field is non-authoritative, and will only manage the labels present in your configuration.
Please refer to the field 'effective_labels' for all of the labels present on the resource.</rdfs:comment>
    <rdfs:domain rdf:resource="http://example.org/onto/class/google_edgenetwork_interconnect_attachment"/>
    <rdfs:range rdf:resource="http://www.w3.org/2001/XMLSchema#string"/>
  </owl:DatatypeProperty>
  <owl:DatatypeProperty rdf:about="http://example.org/onto/prop/google_edgenetwork_interconnect_attachment_location">
    <rdfs:label>location</rdfs:label>
    <rdfs:comment>The Google Cloud region to which the target Distributed Cloud Edge zone belongs.</rdfs:comment>
    <rdfs:domain rdf:resource="http://example.org/onto/class/google_edgenetwork_interconnect_attachment"/>
    <rdfs:range rdf:resource="http://www.w3.org/2001/XMLSchema#string"/>
  </owl:DatatypeProperty>
  <owl:DatatypeProperty rdf:about="http://example.org/onto/prop/google_edgenetwork_interconnect_attachment_mtu">
    <rdfs:label>mtu</rdfs:label>
    <rdfs:comment>IP (L3) MTU value of the virtual edge cloud. Default value is '1500'. Possible values are: '1500', '9000'.</rdfs:comment>
    <rdfs:domain rdf:resource="http://example.org/onto/class/google_edgenetwork_interconnect_attachment"/>
    <rdfs:range rdf:resource="http://www.w3.org/2001/XMLSchema#string"/>
  </owl:DatatypeProperty>
  <owl:DatatypeProperty rdf:about="http://example.org/onto/prop/google_edgenetwork_interconnect_attachment_name">
    <rdfs:label>name</rdfs:label>
    <rdfs:comment>The canonical name of this resource, with format
'projects/{{project}}/locations/{{location}}/zones/{{zone}}/interconnectAttachments/{{interconnect_attachment_id}}'</rdfs:comment>
    <rdfs:domain rdf:resource="http://example.org/onto/class/google_edgenetwork_interconnect_attachment"/>
    <rdfs:range rdf:resource="http://www.w3.org/2001/XMLSchema#string"/>
  </owl:DatatypeProperty>
  <owl:DatatypeProperty rdf:about="http://example.org/onto/prop/google_edgenetwork_interconnect_attachment_network">
    <rdfs:label>network</rdfs:label>
    <rdfs:comment>The ID of the network to which this interconnect attachment belongs.
Must be of the form: 'projects/{{project}}/locations/{{location}}/zones/{{zone}}/networks/{{network_id}}'</rdfs:comment>
    <rdfs:domain rdf:resource="http://example.org/onto/class/google_edgenetwork_interconnect_attachment"/>
    <rdfs:range rdf:resource="http://www.w3.org/2001/XMLSchema#string"/>
  </owl:DatatypeProperty>
  <owl:DatatypeProperty rdf:about="http://example.org/onto/prop/google_edgenetwork_interconnect_attachment_project">
    <rdfs:label>project</rdfs:label>
    <rdfs:domain rdf:resource="http://example.org/onto/class/google_edgenetwork_interconnect_attachment"/>
    <rdfs:range rdf:resource="http://www.w3.org/2001/XMLSchema#string"/>
  </owl:DatatypeProperty>
  <owl:DatatypeProperty rdf:about="http://example.org/onto/prop/google_edgenetwork_interconnect_attachment_terraform_labels">
    <rdfs:label>terraform_labels</rdfs:label>
    <rdfs:comment>The combination of labels configured directly on the resource
 and default labels configured on the provider.</rdfs:comment>
    <rdfs:domain rdf:resource="http://example.org/onto/class/google_edgenetwork_interconnect_attachment"/>
    <rdfs:range rdf:resource="http://www.w3.org/2001/XMLSchema#string"/>
  </owl:DatatypeProperty>
  <owl:DatatypeProperty rdf:about="http://example.org/onto/prop/google_edgenetwork_interconnect_attachment_update_time">
    <rdfs:label>update_time</rdfs:label>
    <rdfs:comment>The time when the resource was last updated.
A timestamp in RFC3339 UTC "Zulu" format, with nanosecond resolution and up to nine
fractional digits. Examples: '2014-10-02T15:01:23Z' and '2014-10-02T15:01:23.045123456Z'.</rdfs:comment>
    <rdfs:domain rdf:resource="http://example.org/onto/class/google_edgenetwork_interconnect_attachment"/>
    <rdfs:range rdf:resource="http://www.w3.org/2001/XMLSchema#string"/>
  </owl:DatatypeProperty>
  <owl:DatatypeProperty rdf:about="http://example.org/onto/prop/google_edgenetwork_interconnect_attachment_vlan_id">
    <rdfs:label>vlan_id</rdfs:label>
    <rdfs:comment>VLAN ID provided by user. Must be site-wise unique.</rdfs:comment>
    <rdfs:domain rdf:resource="http://example.org/onto/class/google_edgenetwork_interconnect_attachment"/>
    <rdfs:range rdf:resource="http://www.w3.org/2001/XMLSchema#string"/>
  </owl:DatatypeProperty>
  <owl:DatatypeProperty rdf:about="http://example.org/onto/prop/google_edgenetwork_interconnect_attachment_zone">
    <rdfs:label>zone</rdfs:label>
    <rdfs:comment>The name of the target Distributed Cloud Edge zone.</rdfs:comment>
    <rdfs:domain rdf:resource="http://example.org/onto/class/google_edgenetwork_interconnect_attachment"/>
    <rdfs:range rdf:resource="http://www.w3.org/2001/XMLSchema#string"/>
  </owl:DatatypeProperty>
  <owl:DatatypeProperty rdf:about="http://example.org/onto/prop/google_edgenetwork_interconnect_attachment_create">
    <rdfs:label>create</rdfs:label>
    <rdfs:domain rdf:resource="http://example.org/onto/class/google_edgenetwork_interconnect_attachment"/>
    <rdfs:range rdf:resource="http://www.w3.org/2001/XMLSchema#string"/>
  </owl:DatatypeProperty>
  <owl:DatatypeProperty rdf:about="http://example.org/onto/prop/google_edgenetwork_interconnect_attachment_delete">
    <rdfs:label>delete</rdfs:label>
    <rdfs:domain rdf:resource="http://example.org/onto/class/google_edgenetwork_interconnect_attachment"/>
    <rdfs:range rdf:resource="http://www.w3.org/2001/XMLSchema#string"/>
  </owl:DatatypeProperty>
  <owl:DatatypeProperty rdf:about="http://example.org/onto/prop/google_edgenetwork_interconnect_attachment_update">
    <rdfs:label>update</rdfs:label>
    <rdfs:domain rdf:resource="http://example.org/onto/class/google_edgenetwork_interconnect_attachment"/>
    <rdfs:range rdf:resource="http://www.w3.org/2001/XMLSchema#string"/>
  </owl:DatatypeProperty>
</rdf:RDF>
