<?xml version="1.0" encoding="UTF-8"?>
<rdf:RDF
  xmlns:rdf="http://www.w3.org/1999/02/22-rdf-syntax-ns#"
  xmlns:rdfs="http://www.w3.org/2000/01/rdf-schema#"
  xmlns:owl="http://www.w3.org/2002/07/owl#"
  xmlns:xsd="http://www.w3.org/2001/XMLSchema#"
  xml:base="http://example.org/onto/">
  <owl:Class rdf:about="http://example.org/onto/class/google_dialogflow_cx_entity_type">
    <rdfs:label>google_dialogflow_cx_entity_type</rdfs:label>
    <rdfs:comment>#
#     ***     AUTO GENERATED CODE    ***    Type: MMv1     ***
#
# ----------------------------------------------------------------------------
#
#     This code is generated by Magic Modules using the following:
#
#     Configuration: https:#github.com/GoogleCloudPlatform/magic-modules/tree/main/mmv1/products/dialogflowcx/EntityType.yaml
#     Template:      https:#github.com/GoogleCloudPlatform/magic-modules/tree/main/mmv1/templates/terraform/resource.html.markdown.tmpl
#
#     DO NOT EDIT this file directly. Any changes made to this file will be
#     overwritten during the next generation cycle.
#
# ----------------------------------------------------------------------------
subcategory: "Dialogflow CX"
description: |-
  Entities are extracted from user input and represent parameters that are meaningful to your application.
---</rdfs:comment>
  </owl:Class>
  <owl:DatatypeProperty rdf:about="http://example.org/onto/prop/google_dialogflow_cx_entity_type_auto_expansion_mode">
    <rdfs:label>auto_expansion_mode</rdfs:label>
    <rdfs:comment>Represents kinds of entities.
* AUTO_EXPANSION_MODE_UNSPECIFIED: Auto expansion disabled for the entity.
* AUTO_EXPANSION_MODE_DEFAULT: Allows an agent to recognize values that have not been explicitly listed in the entity. Possible values: ["AUTO_EXPANSION_MODE_DEFAULT", "AUTO_EXPANSION_MODE_UNSPECIFIED"]</rdfs:comment>
    <rdfs:domain rdf:resource="http://example.org/onto/class/google_dialogflow_cx_entity_type"/>
    <rdfs:range rdf:resource="http://www.w3.org/2001/XMLSchema#string"/>
  </owl:DatatypeProperty>
  <owl:DatatypeProperty rdf:about="http://example.org/onto/prop/google_dialogflow_cx_entity_type_display_name">
    <rdfs:label>display_name</rdfs:label>
    <rdfs:comment>The human-readable name of the entity type, unique within the agent.</rdfs:comment>
    <rdfs:domain rdf:resource="http://example.org/onto/class/google_dialogflow_cx_entity_type"/>
    <rdfs:range rdf:resource="http://www.w3.org/2001/XMLSchema#string"/>
  </owl:DatatypeProperty>
  <owl:DatatypeProperty rdf:about="http://example.org/onto/prop/google_dialogflow_cx_entity_type_enable_fuzzy_extraction">
    <rdfs:label>enable_fuzzy_extraction</rdfs:label>
    <rdfs:comment>Enables fuzzy entity extraction during classification.</rdfs:comment>
    <rdfs:domain rdf:resource="http://example.org/onto/class/google_dialogflow_cx_entity_type"/>
    <rdfs:range rdf:resource="http://www.w3.org/2001/XMLSchema#string"/>
  </owl:DatatypeProperty>
  <owl:DatatypeProperty rdf:about="http://example.org/onto/prop/google_dialogflow_cx_entity_type_id">
    <rdfs:label>id</rdfs:label>
    <rdfs:domain rdf:resource="http://example.org/onto/class/google_dialogflow_cx_entity_type"/>
    <rdfs:range rdf:resource="http://www.w3.org/2001/XMLSchema#string"/>
  </owl:DatatypeProperty>
  <owl:DatatypeProperty rdf:about="http://example.org/onto/prop/google_dialogflow_cx_entity_type_kind">
    <rdfs:label>kind</rdfs:label>
    <rdfs:comment>Indicates whether the entity type can be automatically expanded.
* KIND_MAP: Map entity types allow mapping of a group of synonyms to a canonical value.
* KIND_LIST: List entity types contain a set of entries that do not map to canonical values. However, list entity types can contain references to other entity types (with or without aliases).
* KIND_REGEXP: Regexp entity types allow to specify regular expressions in entries values. Possible values: ["KIND_MAP", "KIND_LIST", "KIND_REGEXP"]</rdfs:comment>
    <rdfs:domain rdf:resource="http://example.org/onto/class/google_dialogflow_cx_entity_type"/>
    <rdfs:range rdf:resource="http://www.w3.org/2001/XMLSchema#string"/>
  </owl:DatatypeProperty>
  <owl:DatatypeProperty rdf:about="http://example.org/onto/prop/google_dialogflow_cx_entity_type_language_code">
    <rdfs:label>language_code</rdfs:label>
    <rdfs:comment>The language of the following fields in entityType:
EntityType.entities.value
EntityType.entities.synonyms
EntityType.excluded_phrases.value
If not specified, the agent's default language is used. Many languages are supported. Note: languages must be enabled in the agent before they can be used.</rdfs:comment>
    <rdfs:domain rdf:resource="http://example.org/onto/class/google_dialogflow_cx_entity_type"/>
    <rdfs:range rdf:resource="http://www.w3.org/2001/XMLSchema#string"/>
  </owl:DatatypeProperty>
  <owl:DatatypeProperty rdf:about="http://example.org/onto/prop/google_dialogflow_cx_entity_type_name">
    <rdfs:label>name</rdfs:label>
    <rdfs:comment>The unique identifier of the entity type.
Format: projects/<Project ID>/locations/<Location ID>/agents/<Agent ID>/entityTypes/<Entity Type ID>.</rdfs:comment>
    <rdfs:domain rdf:resource="http://example.org/onto/class/google_dialogflow_cx_entity_type"/>
    <rdfs:range rdf:resource="http://www.w3.org/2001/XMLSchema#string"/>
  </owl:DatatypeProperty>
  <owl:DatatypeProperty rdf:about="http://example.org/onto/prop/google_dialogflow_cx_entity_type_parent">
    <rdfs:label>parent</rdfs:label>
    <rdfs:comment>The agent to create a entity type for.
Format: projects/<Project ID>/locations/<Location ID>/agents/<Agent ID>.</rdfs:comment>
    <rdfs:domain rdf:resource="http://example.org/onto/class/google_dialogflow_cx_entity_type"/>
    <rdfs:range rdf:resource="http://www.w3.org/2001/XMLSchema#string"/>
  </owl:DatatypeProperty>
  <owl:DatatypeProperty rdf:about="http://example.org/onto/prop/google_dialogflow_cx_entity_type_redact">
    <rdfs:label>redact</rdfs:label>
    <rdfs:comment>Indicates whether parameters of the entity type should be redacted in log. If redaction is enabled, page parameters and intent parameters referring to the entity type will be replaced by parameter name when logging.</rdfs:comment>
    <rdfs:domain rdf:resource="http://example.org/onto/class/google_dialogflow_cx_entity_type"/>
    <rdfs:range rdf:resource="http://www.w3.org/2001/XMLSchema#string"/>
  </owl:DatatypeProperty>
  <owl:DatatypeProperty rdf:about="http://example.org/onto/prop/google_dialogflow_cx_entity_type_synonyms">
    <rdfs:label>synonyms</rdfs:label>
    <rdfs:comment>A collection of value synonyms. For example, if the entity type is vegetable, and value is scallions, a synonym could be green onions.
For KIND_LIST entity types: This collection must contain exactly one synonym equal to value.</rdfs:comment>
    <rdfs:domain rdf:resource="http://example.org/onto/class/google_dialogflow_cx_entity_type"/>
    <rdfs:range rdf:resource="http://www.w3.org/2001/XMLSchema#string"/>
  </owl:DatatypeProperty>
  <owl:DatatypeProperty rdf:about="http://example.org/onto/prop/google_dialogflow_cx_entity_type_value">
    <rdfs:label>value</rdfs:label>
    <rdfs:comment>The primary value associated with this entity entry. For example, if the entity type is vegetable, the value could be scallions.
For KIND_MAP entity types: A canonical value to be used in place of synonyms.
For KIND_LIST entity types: A string that can contain references to other entity types (with or without aliases).</rdfs:comment>
    <rdfs:domain rdf:resource="http://example.org/onto/class/google_dialogflow_cx_entity_type"/>
    <rdfs:range rdf:resource="http://www.w3.org/2001/XMLSchema#string"/>
  </owl:DatatypeProperty>
  <owl:DatatypeProperty rdf:about="http://example.org/onto/prop/google_dialogflow_cx_entity_type_value">
    <rdfs:label>value</rdfs:label>
    <rdfs:comment>The word or phrase to be excluded.</rdfs:comment>
    <rdfs:domain rdf:resource="http://example.org/onto/class/google_dialogflow_cx_entity_type"/>
    <rdfs:range rdf:resource="http://www.w3.org/2001/XMLSchema#string"/>
  </owl:DatatypeProperty>
  <owl:DatatypeProperty rdf:about="http://example.org/onto/prop/google_dialogflow_cx_entity_type_create">
    <rdfs:label>create</rdfs:label>
    <rdfs:domain rdf:resource="http://example.org/onto/class/google_dialogflow_cx_entity_type"/>
    <rdfs:range rdf:resource="http://www.w3.org/2001/XMLSchema#string"/>
  </owl:DatatypeProperty>
  <owl:DatatypeProperty rdf:about="http://example.org/onto/prop/google_dialogflow_cx_entity_type_delete">
    <rdfs:label>delete</rdfs:label>
    <rdfs:domain rdf:resource="http://example.org/onto/class/google_dialogflow_cx_entity_type"/>
    <rdfs:range rdf:resource="http://www.w3.org/2001/XMLSchema#string"/>
  </owl:DatatypeProperty>
  <owl:DatatypeProperty rdf:about="http://example.org/onto/prop/google_dialogflow_cx_entity_type_update">
    <rdfs:label>update</rdfs:label>
    <rdfs:domain rdf:resource="http://example.org/onto/class/google_dialogflow_cx_entity_type"/>
    <rdfs:range rdf:resource="http://www.w3.org/2001/XMLSchema#string"/>
  </owl:DatatypeProperty>
</rdf:RDF>
