<?xml version="1.0" encoding="UTF-8"?>
<rdf:RDF
  xmlns:rdf="http://www.w3.org/1999/02/22-rdf-syntax-ns#"
  xmlns:rdfs="http://www.w3.org/2000/01/rdf-schema#"
  xmlns:owl="http://www.w3.org/2002/07/owl#"
  xmlns:xsd="http://www.w3.org/2001/XMLSchema#"
  xml:base="http://example.org/onto/">
  <owl:Class rdf:about="http://example.org/onto/class/google_bigtable_instance">
    <rdfs:label>google_bigtable_instance</rdfs:label>
    <rdfs:comment>#
#     ***     AUTO GENERATED CODE    ***    Type: Handwritten     ***
#
# ----------------------------------------------------------------------------
#
#     This code is generated by Magic Modules using the following:
#
#     Source file: https://github.com/GoogleCloudPlatform/magic-modules/tree/main/mmv1/third_party/terraform/website/docs/r/bigtable_instance.html.markdown
#
#     DO NOT EDIT this file directly. Any changes made to this file will be
#     overwritten during the next generation cycle.
#
# ----------------------------------------------------------------------------
subcategory: "Cloud Bigtable"
description: |-
  Creates a Google Bigtable instance.
---</rdfs:comment>
  </owl:Class>
  <owl:DatatypeProperty rdf:about="http://example.org/onto/prop/google_bigtable_instance_deletion_protection">
    <rdfs:label>deletion_protection</rdfs:label>
    <rdfs:comment>When the field is set to true or unset in Terraform state, a terraform apply or terraform destroy that would delete the instance will fail. When the field is set to false, deleting the instance is allowed.</rdfs:comment>
    <rdfs:domain rdf:resource="http://example.org/onto/class/google_bigtable_instance"/>
    <rdfs:range rdf:resource="http://www.w3.org/2001/XMLSchema#string"/>
  </owl:DatatypeProperty>
  <owl:DatatypeProperty rdf:about="http://example.org/onto/prop/google_bigtable_instance_display_name">
    <rdfs:label>display_name</rdfs:label>
    <rdfs:comment>The human-readable display name of the Bigtable instance. Defaults to the instance name.</rdfs:comment>
    <rdfs:domain rdf:resource="http://example.org/onto/class/google_bigtable_instance"/>
    <rdfs:range rdf:resource="http://www.w3.org/2001/XMLSchema#string"/>
  </owl:DatatypeProperty>
  <owl:DatatypeProperty rdf:about="http://example.org/onto/prop/google_bigtable_instance_effective_labels">
    <rdfs:label>effective_labels</rdfs:label>
    <rdfs:comment>All of labels (key/value pairs) present on the resource in GCP, including the labels configured through Terraform, other clients and services.</rdfs:comment>
    <rdfs:domain rdf:resource="http://example.org/onto/class/google_bigtable_instance"/>
    <rdfs:range rdf:resource="http://www.w3.org/2001/XMLSchema#string"/>
  </owl:DatatypeProperty>
  <owl:DatatypeProperty rdf:about="http://example.org/onto/prop/google_bigtable_instance_force_destroy">
    <rdfs:label>force_destroy</rdfs:label>
    <rdfs:comment>When deleting a BigTable instance, this boolean option will delete all backups within the instance.</rdfs:comment>
    <rdfs:domain rdf:resource="http://example.org/onto/class/google_bigtable_instance"/>
    <rdfs:range rdf:resource="http://www.w3.org/2001/XMLSchema#string"/>
  </owl:DatatypeProperty>
  <owl:DatatypeProperty rdf:about="http://example.org/onto/prop/google_bigtable_instance_id">
    <rdfs:label>id</rdfs:label>
    <rdfs:domain rdf:resource="http://example.org/onto/class/google_bigtable_instance"/>
    <rdfs:range rdf:resource="http://www.w3.org/2001/XMLSchema#string"/>
  </owl:DatatypeProperty>
  <owl:DatatypeProperty rdf:about="http://example.org/onto/prop/google_bigtable_instance_instance_type">
    <rdfs:label>instance_type</rdfs:label>
    <rdfs:comment>The instance type to create. One of "DEVELOPMENT" or "PRODUCTION". Defaults to "PRODUCTION".</rdfs:comment>
    <rdfs:domain rdf:resource="http://example.org/onto/class/google_bigtable_instance"/>
    <rdfs:range rdf:resource="http://www.w3.org/2001/XMLSchema#string"/>
  </owl:DatatypeProperty>
  <owl:DatatypeProperty rdf:about="http://example.org/onto/prop/google_bigtable_instance_labels">
    <rdfs:label>labels</rdfs:label>
    <rdfs:comment>A mapping of labels to assign to the resource.
				
				**Note**: This field is non-authoritative, and will only manage the labels present in your configuration.
				Please refer to the field 'effective_labels' for all of the labels present on the resource.</rdfs:comment>
    <rdfs:domain rdf:resource="http://example.org/onto/class/google_bigtable_instance"/>
    <rdfs:range rdf:resource="http://www.w3.org/2001/XMLSchema#string"/>
  </owl:DatatypeProperty>
  <owl:DatatypeProperty rdf:about="http://example.org/onto/prop/google_bigtable_instance_name">
    <rdfs:label>name</rdfs:label>
    <rdfs:comment>The name (also called Instance Id in the Cloud Console) of the Cloud Bigtable instance. Must be 6-33 characters and must only contain hyphens, lowercase letters and numbers.</rdfs:comment>
    <rdfs:domain rdf:resource="http://example.org/onto/class/google_bigtable_instance"/>
    <rdfs:range rdf:resource="http://www.w3.org/2001/XMLSchema#string"/>
  </owl:DatatypeProperty>
  <owl:DatatypeProperty rdf:about="http://example.org/onto/prop/google_bigtable_instance_project">
    <rdfs:label>project</rdfs:label>
    <rdfs:comment>The ID of the project in which the resource belongs. If it is not provided, the provider project is used.</rdfs:comment>
    <rdfs:domain rdf:resource="http://example.org/onto/class/google_bigtable_instance"/>
    <rdfs:range rdf:resource="http://www.w3.org/2001/XMLSchema#string"/>
  </owl:DatatypeProperty>
  <owl:DatatypeProperty rdf:about="http://example.org/onto/prop/google_bigtable_instance_terraform_labels">
    <rdfs:label>terraform_labels</rdfs:label>
    <rdfs:comment>The combination of labels configured directly on the resource and default labels configured on the provider.</rdfs:comment>
    <rdfs:domain rdf:resource="http://example.org/onto/class/google_bigtable_instance"/>
    <rdfs:range rdf:resource="http://www.w3.org/2001/XMLSchema#string"/>
  </owl:DatatypeProperty>
  <owl:DatatypeProperty rdf:about="http://example.org/onto/prop/google_bigtable_instance_cluster_id">
    <rdfs:label>cluster_id</rdfs:label>
    <rdfs:comment>The ID of the Cloud Bigtable cluster. Must be 6-30 characters and must only contain hyphens, lowercase letters and numbers.</rdfs:comment>
    <rdfs:domain rdf:resource="http://example.org/onto/class/google_bigtable_instance"/>
    <rdfs:range rdf:resource="http://www.w3.org/2001/XMLSchema#string"/>
  </owl:DatatypeProperty>
  <owl:DatatypeProperty rdf:about="http://example.org/onto/prop/google_bigtable_instance_kms_key_name">
    <rdfs:label>kms_key_name</rdfs:label>
    <rdfs:comment>Describes the Cloud KMS encryption key that will be used to protect the destination Bigtable cluster. The requirements for this key are: 1) The Cloud Bigtable service account associated with the project that contains this cluster must be granted the cloudkms.cryptoKeyEncrypterDecrypter role on the CMEK key. 2) Only regional keys can be used and the region of the CMEK key must match the region of the cluster. 3) All clusters within an instance must use the same CMEK key. Values are of the form projects/{project}/locations/{location}/keyRings/{keyring}/cryptoKeys/{key}</rdfs:comment>
    <rdfs:domain rdf:resource="http://example.org/onto/class/google_bigtable_instance"/>
    <rdfs:range rdf:resource="http://www.w3.org/2001/XMLSchema#string"/>
  </owl:DatatypeProperty>
  <owl:DatatypeProperty rdf:about="http://example.org/onto/prop/google_bigtable_instance_node_scaling_factor">
    <rdfs:label>node_scaling_factor</rdfs:label>
    <rdfs:comment>The node scaling factor of this cluster. One of "NodeScalingFactor1X" or "NodeScalingFactor2X". Defaults to "NodeScalingFactor1X".</rdfs:comment>
    <rdfs:domain rdf:resource="http://example.org/onto/class/google_bigtable_instance"/>
    <rdfs:range rdf:resource="http://www.w3.org/2001/XMLSchema#string"/>
  </owl:DatatypeProperty>
  <owl:DatatypeProperty rdf:about="http://example.org/onto/prop/google_bigtable_instance_num_nodes">
    <rdfs:label>num_nodes</rdfs:label>
    <rdfs:comment>The number of nodes in the cluster. If no value is set, Cloud Bigtable automatically allocates nodes based on your data footprint and optimized for 50% storage utilization.</rdfs:comment>
    <rdfs:domain rdf:resource="http://example.org/onto/class/google_bigtable_instance"/>
    <rdfs:range rdf:resource="http://www.w3.org/2001/XMLSchema#string"/>
  </owl:DatatypeProperty>
  <owl:DatatypeProperty rdf:about="http://example.org/onto/prop/google_bigtable_instance_state">
    <rdfs:label>state</rdfs:label>
    <rdfs:comment>The state of the cluster</rdfs:comment>
    <rdfs:domain rdf:resource="http://example.org/onto/class/google_bigtable_instance"/>
    <rdfs:range rdf:resource="http://www.w3.org/2001/XMLSchema#string"/>
  </owl:DatatypeProperty>
  <owl:DatatypeProperty rdf:about="http://example.org/onto/prop/google_bigtable_instance_storage_type">
    <rdfs:label>storage_type</rdfs:label>
    <rdfs:comment>The storage type to use. One of "SSD" or "HDD". Defaults to "SSD".</rdfs:comment>
    <rdfs:domain rdf:resource="http://example.org/onto/class/google_bigtable_instance"/>
    <rdfs:range rdf:resource="http://www.w3.org/2001/XMLSchema#string"/>
  </owl:DatatypeProperty>
  <owl:DatatypeProperty rdf:about="http://example.org/onto/prop/google_bigtable_instance_zone">
    <rdfs:label>zone</rdfs:label>
    <rdfs:comment>The zone to create the Cloud Bigtable cluster in. Each cluster must have a different zone in the same region. Zones that support Bigtable instances are noted on the Cloud Bigtable locations page.</rdfs:comment>
    <rdfs:domain rdf:resource="http://example.org/onto/class/google_bigtable_instance"/>
    <rdfs:range rdf:resource="http://www.w3.org/2001/XMLSchema#string"/>
  </owl:DatatypeProperty>
  <owl:DatatypeProperty rdf:about="http://example.org/onto/prop/google_bigtable_instance_cpu_target">
    <rdfs:label>cpu_target</rdfs:label>
    <rdfs:comment>The target CPU utilization for autoscaling. Value must be between 10 and 80.</rdfs:comment>
    <rdfs:domain rdf:resource="http://example.org/onto/class/google_bigtable_instance"/>
    <rdfs:range rdf:resource="http://www.w3.org/2001/XMLSchema#string"/>
  </owl:DatatypeProperty>
  <owl:DatatypeProperty rdf:about="http://example.org/onto/prop/google_bigtable_instance_max_nodes">
    <rdfs:label>max_nodes</rdfs:label>
    <rdfs:comment>The maximum number of nodes for autoscaling.</rdfs:comment>
    <rdfs:domain rdf:resource="http://example.org/onto/class/google_bigtable_instance"/>
    <rdfs:range rdf:resource="http://www.w3.org/2001/XMLSchema#string"/>
  </owl:DatatypeProperty>
  <owl:DatatypeProperty rdf:about="http://example.org/onto/prop/google_bigtable_instance_min_nodes">
    <rdfs:label>min_nodes</rdfs:label>
    <rdfs:comment>The minimum number of nodes for autoscaling.</rdfs:comment>
    <rdfs:domain rdf:resource="http://example.org/onto/class/google_bigtable_instance"/>
    <rdfs:range rdf:resource="http://www.w3.org/2001/XMLSchema#string"/>
  </owl:DatatypeProperty>
  <owl:DatatypeProperty rdf:about="http://example.org/onto/prop/google_bigtable_instance_storage_target">
    <rdfs:label>storage_target</rdfs:label>
    <rdfs:comment>The target storage utilization for autoscaling, in GB, for each node in a cluster. This number is limited between 2560 (2.5TiB) and 5120 (5TiB) for a SSD cluster and between 8192 (8TiB) and 16384 (16 TiB) for an HDD cluster. If not set, whatever is already set for the cluster will not change, or if the cluster is just being created, it will use the default value of 2560 for SSD clusters and 8192 for HDD clusters.</rdfs:comment>
    <rdfs:domain rdf:resource="http://example.org/onto/class/google_bigtable_instance"/>
    <rdfs:range rdf:resource="http://www.w3.org/2001/XMLSchema#string"/>
  </owl:DatatypeProperty>
  <owl:DatatypeProperty rdf:about="http://example.org/onto/prop/google_bigtable_instance_create">
    <rdfs:label>create</rdfs:label>
    <rdfs:domain rdf:resource="http://example.org/onto/class/google_bigtable_instance"/>
    <rdfs:range rdf:resource="http://www.w3.org/2001/XMLSchema#string"/>
  </owl:DatatypeProperty>
  <owl:DatatypeProperty rdf:about="http://example.org/onto/prop/google_bigtable_instance_read">
    <rdfs:label>read</rdfs:label>
    <rdfs:domain rdf:resource="http://example.org/onto/class/google_bigtable_instance"/>
    <rdfs:range rdf:resource="http://www.w3.org/2001/XMLSchema#string"/>
  </owl:DatatypeProperty>
  <owl:DatatypeProperty rdf:about="http://example.org/onto/prop/google_bigtable_instance_update">
    <rdfs:label>update</rdfs:label>
    <rdfs:domain rdf:resource="http://example.org/onto/class/google_bigtable_instance"/>
    <rdfs:range rdf:resource="http://www.w3.org/2001/XMLSchema#string"/>
  </owl:DatatypeProperty>
</rdf:RDF>
