<?xml version="1.0" encoding="UTF-8"?>
<rdf:RDF
  xmlns:rdf="http://www.w3.org/1999/02/22-rdf-syntax-ns#"
  xmlns:rdfs="http://www.w3.org/2000/01/rdf-schema#"
  xmlns:owl="http://www.w3.org/2002/07/owl#"
  xmlns:xsd="http://www.w3.org/2001/XMLSchema#"
  xml:base="http://example.org/onto/">
  <owl:Class rdf:about="http://example.org/onto/class/google_network_security_gateway_security_policy">
    <rdfs:label>google_network_security_gateway_security_policy</rdfs:label>
    <rdfs:comment>#
#     ***     AUTO GENERATED CODE    ***    Type: MMv1     ***
#
# ----------------------------------------------------------------------------
#
#     This code is generated by Magic Modules using the following:
#
#     Configuration: https:#github.com/GoogleCloudPlatform/magic-modules/tree/main/mmv1/products/networksecurity/GatewaySecurityPolicy.yaml
#     Template:      https:#github.com/GoogleCloudPlatform/magic-modules/tree/main/mmv1/templates/terraform/resource.html.markdown.tmpl
#
#     DO NOT EDIT this file directly. Any changes made to this file will be
#     overwritten during the next generation cycle.
#
# ----------------------------------------------------------------------------
subcategory: "Network Security"
description: |-
  The GatewaySecurityPolicy resource contains a collection of GatewaySecurityPolicyRules and associated metadata.
---</rdfs:comment>
  </owl:Class>
  <owl:DatatypeProperty rdf:about="http://example.org/onto/prop/google_network_security_gateway_security_policy_create_time">
    <rdfs:label>create_time</rdfs:label>
    <rdfs:comment>The timestamp when the resource was created.
A timestamp in RFC3339 UTC "Zulu" format, with nanosecond resolution and up to nine fractional digits.
Examples: "2014-10-02T15:01:23Z" and "2014-10-02T15:01:23.045123456Z"</rdfs:comment>
    <rdfs:domain rdf:resource="http://example.org/onto/class/google_network_security_gateway_security_policy"/>
    <rdfs:range rdf:resource="http://www.w3.org/2001/XMLSchema#string"/>
  </owl:DatatypeProperty>
  <owl:DatatypeProperty rdf:about="http://example.org/onto/prop/google_network_security_gateway_security_policy_description">
    <rdfs:label>description</rdfs:label>
    <rdfs:comment>A free-text description of the resource. Max length 1024 characters.</rdfs:comment>
    <rdfs:domain rdf:resource="http://example.org/onto/class/google_network_security_gateway_security_policy"/>
    <rdfs:range rdf:resource="http://www.w3.org/2001/XMLSchema#string"/>
  </owl:DatatypeProperty>
  <owl:DatatypeProperty rdf:about="http://example.org/onto/prop/google_network_security_gateway_security_policy_id">
    <rdfs:label>id</rdfs:label>
    <rdfs:domain rdf:resource="http://example.org/onto/class/google_network_security_gateway_security_policy"/>
    <rdfs:range rdf:resource="http://www.w3.org/2001/XMLSchema#string"/>
  </owl:DatatypeProperty>
  <owl:DatatypeProperty rdf:about="http://example.org/onto/prop/google_network_security_gateway_security_policy_location">
    <rdfs:label>location</rdfs:label>
    <rdfs:comment>The location of the gateway security policy.
The default value is 'global'.</rdfs:comment>
    <rdfs:domain rdf:resource="http://example.org/onto/class/google_network_security_gateway_security_policy"/>
    <rdfs:range rdf:resource="http://www.w3.org/2001/XMLSchema#string"/>
  </owl:DatatypeProperty>
  <owl:DatatypeProperty rdf:about="http://example.org/onto/prop/google_network_security_gateway_security_policy_name">
    <rdfs:label>name</rdfs:label>
    <rdfs:comment>Name of the resource. Name is of the form projects/{project}/locations/{location}/gatewaySecurityPolicies/{gatewaySecurityPolicy}
gatewaySecurityPolicy should match the pattern:(^a-z?$).</rdfs:comment>
    <rdfs:domain rdf:resource="http://example.org/onto/class/google_network_security_gateway_security_policy"/>
    <rdfs:range rdf:resource="http://www.w3.org/2001/XMLSchema#string"/>
  </owl:DatatypeProperty>
  <owl:DatatypeProperty rdf:about="http://example.org/onto/prop/google_network_security_gateway_security_policy_project">
    <rdfs:label>project</rdfs:label>
    <rdfs:domain rdf:resource="http://example.org/onto/class/google_network_security_gateway_security_policy"/>
    <rdfs:range rdf:resource="http://www.w3.org/2001/XMLSchema#string"/>
  </owl:DatatypeProperty>
  <owl:DatatypeProperty rdf:about="http://example.org/onto/prop/google_network_security_gateway_security_policy_self_link">
    <rdfs:label>self_link</rdfs:label>
    <rdfs:comment>Server-defined URL of this resource.</rdfs:comment>
    <rdfs:domain rdf:resource="http://example.org/onto/class/google_network_security_gateway_security_policy"/>
    <rdfs:range rdf:resource="http://www.w3.org/2001/XMLSchema#string"/>
  </owl:DatatypeProperty>
  <owl:DatatypeProperty rdf:about="http://example.org/onto/prop/google_network_security_gateway_security_policy_tls_inspection_policy">
    <rdfs:label>tls_inspection_policy</rdfs:label>
    <rdfs:comment>Name of a TlsInspectionPolicy resource that defines how TLS inspection is performed for any rule that enables it.</rdfs:comment>
    <rdfs:domain rdf:resource="http://example.org/onto/class/google_network_security_gateway_security_policy"/>
    <rdfs:range rdf:resource="http://www.w3.org/2001/XMLSchema#string"/>
  </owl:DatatypeProperty>
  <owl:DatatypeProperty rdf:about="http://example.org/onto/prop/google_network_security_gateway_security_policy_update_time">
    <rdfs:label>update_time</rdfs:label>
    <rdfs:comment>The timestamp when the resource was updated.
A timestamp in RFC3339 UTC "Zulu" format, with nanosecond resolution and up to nine fractional digits.
Examples: "2014-10-02T15:01:23Z" and "2014-10-02T15:01:23.045123456Z".</rdfs:comment>
    <rdfs:domain rdf:resource="http://example.org/onto/class/google_network_security_gateway_security_policy"/>
    <rdfs:range rdf:resource="http://www.w3.org/2001/XMLSchema#string"/>
  </owl:DatatypeProperty>
  <owl:DatatypeProperty rdf:about="http://example.org/onto/prop/google_network_security_gateway_security_policy_create">
    <rdfs:label>create</rdfs:label>
    <rdfs:domain rdf:resource="http://example.org/onto/class/google_network_security_gateway_security_policy"/>
    <rdfs:range rdf:resource="http://www.w3.org/2001/XMLSchema#string"/>
  </owl:DatatypeProperty>
  <owl:DatatypeProperty rdf:about="http://example.org/onto/prop/google_network_security_gateway_security_policy_delete">
    <rdfs:label>delete</rdfs:label>
    <rdfs:domain rdf:resource="http://example.org/onto/class/google_network_security_gateway_security_policy"/>
    <rdfs:range rdf:resource="http://www.w3.org/2001/XMLSchema#string"/>
  </owl:DatatypeProperty>
  <owl:DatatypeProperty rdf:about="http://example.org/onto/prop/google_network_security_gateway_security_policy_update">
    <rdfs:label>update</rdfs:label>
    <rdfs:domain rdf:resource="http://example.org/onto/class/google_network_security_gateway_security_policy"/>
    <rdfs:range rdf:resource="http://www.w3.org/2001/XMLSchema#string"/>
  </owl:DatatypeProperty>
</rdf:RDF>
