<?xml version="1.0" encoding="UTF-8"?>
<rdf:RDF
  xmlns:rdf="http://www.w3.org/1999/02/22-rdf-syntax-ns#"
  xmlns:rdfs="http://www.w3.org/2000/01/rdf-schema#"
  xmlns:owl="http://www.w3.org/2002/07/owl#"
  xmlns:xsd="http://www.w3.org/2001/XMLSchema#"
  xml:base="http://example.org/onto/">
  <owl:Class rdf:about="http://example.org/onto/class/google_managed_kafka_connector">
    <rdfs:label>google_managed_kafka_connector</rdfs:label>
    <rdfs:comment>#
#     ***     AUTO GENERATED CODE    ***    Type: MMv1     ***
#
# ----------------------------------------------------------------------------
#
#     This code is generated by Magic Modules using the following:
#
#     Configuration: https:#github.com/GoogleCloudPlatform/magic-modules/tree/main/mmv1/products/managedkafka/Connector.yaml
#     Template:      https:#github.com/GoogleCloudPlatform/magic-modules/tree/main/mmv1/templates/terraform/resource.html.markdown.tmpl
#
#     DO NOT EDIT this file directly. Any changes made to this file will be
#     overwritten during the next generation cycle.
#
# ----------------------------------------------------------------------------
subcategory: "Managed Kafka"
description: |-
  A Managed Service for Kafka Connect Connectors.
---</rdfs:comment>
  </owl:Class>
  <owl:DatatypeProperty rdf:about="http://example.org/onto/prop/google_managed_kafka_connector_configs">
    <rdfs:label>configs</rdfs:label>
    <rdfs:comment>Connector config as keys/values. The keys of the map are connector property names, for example: 'connector.class', 'tasks.max', 'key.converter'.</rdfs:comment>
    <rdfs:domain rdf:resource="http://example.org/onto/class/google_managed_kafka_connector"/>
    <rdfs:range rdf:resource="http://www.w3.org/2001/XMLSchema#string"/>
  </owl:DatatypeProperty>
  <owl:DatatypeProperty rdf:about="http://example.org/onto/prop/google_managed_kafka_connector_connect_cluster">
    <rdfs:label>connect_cluster</rdfs:label>
    <rdfs:comment>The connect cluster name.</rdfs:comment>
    <rdfs:domain rdf:resource="http://example.org/onto/class/google_managed_kafka_connector"/>
    <rdfs:range rdf:resource="http://www.w3.org/2001/XMLSchema#string"/>
  </owl:DatatypeProperty>
  <owl:DatatypeProperty rdf:about="http://example.org/onto/prop/google_managed_kafka_connector_connector_id">
    <rdfs:label>connector_id</rdfs:label>
    <rdfs:comment>The ID to use for the connector, which will become the final component of the connector's name. This value is structured like: 'my-connector-id'.</rdfs:comment>
    <rdfs:domain rdf:resource="http://example.org/onto/class/google_managed_kafka_connector"/>
    <rdfs:range rdf:resource="http://www.w3.org/2001/XMLSchema#string"/>
  </owl:DatatypeProperty>
  <owl:DatatypeProperty rdf:about="http://example.org/onto/prop/google_managed_kafka_connector_id">
    <rdfs:label>id</rdfs:label>
    <rdfs:domain rdf:resource="http://example.org/onto/class/google_managed_kafka_connector"/>
    <rdfs:range rdf:resource="http://www.w3.org/2001/XMLSchema#string"/>
  </owl:DatatypeProperty>
  <owl:DatatypeProperty rdf:about="http://example.org/onto/prop/google_managed_kafka_connector_location">
    <rdfs:label>location</rdfs:label>
    <rdfs:comment>ID of the location of the Kafka Connect resource. See https://cloud.google.com/managed-kafka/docs/locations for a list of supported locations.</rdfs:comment>
    <rdfs:domain rdf:resource="http://example.org/onto/class/google_managed_kafka_connector"/>
    <rdfs:range rdf:resource="http://www.w3.org/2001/XMLSchema#string"/>
  </owl:DatatypeProperty>
  <owl:DatatypeProperty rdf:about="http://example.org/onto/prop/google_managed_kafka_connector_name">
    <rdfs:label>name</rdfs:label>
    <rdfs:comment>The name of the connector. The 'connector' segment is used when connecting directly to the connect cluster. Structured like: 'projects/PROJECT_ID/locations/LOCATION/connectClusters/CONNECT_CLUSTER/connectors/CONNECTOR_ID'.</rdfs:comment>
    <rdfs:domain rdf:resource="http://example.org/onto/class/google_managed_kafka_connector"/>
    <rdfs:range rdf:resource="http://www.w3.org/2001/XMLSchema#string"/>
  </owl:DatatypeProperty>
  <owl:DatatypeProperty rdf:about="http://example.org/onto/prop/google_managed_kafka_connector_project">
    <rdfs:label>project</rdfs:label>
    <rdfs:domain rdf:resource="http://example.org/onto/class/google_managed_kafka_connector"/>
    <rdfs:range rdf:resource="http://www.w3.org/2001/XMLSchema#string"/>
  </owl:DatatypeProperty>
  <owl:DatatypeProperty rdf:about="http://example.org/onto/prop/google_managed_kafka_connector_state">
    <rdfs:label>state</rdfs:label>
    <rdfs:comment>The current state of the connect. Possible values: 'STATE_UNSPECIFIED', 'UNASSIGNED', 'RUNNING', 'PAUSED', 'FAILED', 'RESTARTING', and 'STOPPED'.</rdfs:comment>
    <rdfs:domain rdf:resource="http://example.org/onto/class/google_managed_kafka_connector"/>
    <rdfs:range rdf:resource="http://www.w3.org/2001/XMLSchema#string"/>
  </owl:DatatypeProperty>
  <owl:DatatypeProperty rdf:about="http://example.org/onto/prop/google_managed_kafka_connector_maximum_backoff">
    <rdfs:label>maximum_backoff</rdfs:label>
    <rdfs:comment>The maximum amount of time to wait before retrying a failed task. This sets an upper bound for the backoff delay.
A duration in seconds with up to nine fractional digits, terminated by 's'. Example: "3.5s".</rdfs:comment>
    <rdfs:domain rdf:resource="http://example.org/onto/class/google_managed_kafka_connector"/>
    <rdfs:range rdf:resource="http://www.w3.org/2001/XMLSchema#string"/>
  </owl:DatatypeProperty>
  <owl:DatatypeProperty rdf:about="http://example.org/onto/prop/google_managed_kafka_connector_minimum_backoff">
    <rdfs:label>minimum_backoff</rdfs:label>
    <rdfs:comment>The minimum amount of time to wait before retrying a failed task. This sets a lower bound for the backoff delay.
A duration in seconds with up to nine fractional digits, terminated by 's'. Example: "3.5s".</rdfs:comment>
    <rdfs:domain rdf:resource="http://example.org/onto/class/google_managed_kafka_connector"/>
    <rdfs:range rdf:resource="http://www.w3.org/2001/XMLSchema#string"/>
  </owl:DatatypeProperty>
  <owl:DatatypeProperty rdf:about="http://example.org/onto/prop/google_managed_kafka_connector_create">
    <rdfs:label>create</rdfs:label>
    <rdfs:domain rdf:resource="http://example.org/onto/class/google_managed_kafka_connector"/>
    <rdfs:range rdf:resource="http://www.w3.org/2001/XMLSchema#string"/>
  </owl:DatatypeProperty>
  <owl:DatatypeProperty rdf:about="http://example.org/onto/prop/google_managed_kafka_connector_delete">
    <rdfs:label>delete</rdfs:label>
    <rdfs:domain rdf:resource="http://example.org/onto/class/google_managed_kafka_connector"/>
    <rdfs:range rdf:resource="http://www.w3.org/2001/XMLSchema#string"/>
  </owl:DatatypeProperty>
  <owl:DatatypeProperty rdf:about="http://example.org/onto/prop/google_managed_kafka_connector_update">
    <rdfs:label>update</rdfs:label>
    <rdfs:domain rdf:resource="http://example.org/onto/class/google_managed_kafka_connector"/>
    <rdfs:range rdf:resource="http://www.w3.org/2001/XMLSchema#string"/>
  </owl:DatatypeProperty>
</rdf:RDF>
