<?xml version="1.0" encoding="UTF-8"?>
<rdf:RDF
  xmlns:rdf="http://www.w3.org/1999/02/22-rdf-syntax-ns#"
  xmlns:rdfs="http://www.w3.org/2000/01/rdf-schema#"
  xmlns:owl="http://www.w3.org/2002/07/owl#"
  xmlns:xsd="http://www.w3.org/2001/XMLSchema#"
  xml:base="http://example.org/onto/">
  <owl:Class rdf:about="http://example.org/onto/class/google_dataplex_entry">
    <rdfs:label>google_dataplex_entry</rdfs:label>
    <rdfs:comment>#
#     ***     AUTO GENERATED CODE    ***    Type: MMv1     ***
#
# ----------------------------------------------------------------------------
#
#     This code is generated by Magic Modules using the following:
#
#     Configuration: https:#github.com/GoogleCloudPlatform/magic-modules/tree/main/mmv1/products/dataplex/Entry.yaml
#     Template:      https:#github.com/GoogleCloudPlatform/magic-modules/tree/main/mmv1/templates/terraform/resource.html.markdown.tmpl
#
#     DO NOT EDIT this file directly. Any changes made to this file will be
#     overwritten during the next generation cycle.
#
# ----------------------------------------------------------------------------
subcategory: "Dataplex"
description: |-
  An entry represents a data asset for which you capture metadata, such as a BigQuery table.
---</rdfs:comment>
  </owl:Class>
  <owl:DatatypeProperty rdf:about="http://example.org/onto/prop/google_dataplex_entry_create_time">
    <rdfs:label>create_time</rdfs:label>
    <rdfs:comment>The time when the Entry was created in Dataplex.</rdfs:comment>
    <rdfs:domain rdf:resource="http://example.org/onto/class/google_dataplex_entry"/>
    <rdfs:range rdf:resource="http://www.w3.org/2001/XMLSchema#string"/>
  </owl:DatatypeProperty>
  <owl:DatatypeProperty rdf:about="http://example.org/onto/prop/google_dataplex_entry_entry_group_id">
    <rdfs:label>entry_group_id</rdfs:label>
    <rdfs:comment>The entry group id of the entry group the entry will be created in.</rdfs:comment>
    <rdfs:domain rdf:resource="http://example.org/onto/class/google_dataplex_entry"/>
    <rdfs:range rdf:resource="http://www.w3.org/2001/XMLSchema#string"/>
  </owl:DatatypeProperty>
  <owl:DatatypeProperty rdf:about="http://example.org/onto/prop/google_dataplex_entry_entry_id">
    <rdfs:label>entry_id</rdfs:label>
    <rdfs:comment>The entry id of the entry.</rdfs:comment>
    <rdfs:domain rdf:resource="http://example.org/onto/class/google_dataplex_entry"/>
    <rdfs:range rdf:resource="http://www.w3.org/2001/XMLSchema#string"/>
  </owl:DatatypeProperty>
  <owl:DatatypeProperty rdf:about="http://example.org/onto/prop/google_dataplex_entry_entry_type">
    <rdfs:label>entry_type</rdfs:label>
    <rdfs:comment>The relative resource name of the entry type that was used to create this entry, in the format projects/{project_number}/locations/{locationId}/entryTypes/{entryTypeId}.</rdfs:comment>
    <rdfs:domain rdf:resource="http://example.org/onto/class/google_dataplex_entry"/>
    <rdfs:range rdf:resource="http://www.w3.org/2001/XMLSchema#string"/>
  </owl:DatatypeProperty>
  <owl:DatatypeProperty rdf:about="http://example.org/onto/prop/google_dataplex_entry_fully_qualified_name">
    <rdfs:label>fully_qualified_name</rdfs:label>
    <rdfs:comment>A name for the entry that can be referenced by an external system. For more information, see https://cloud.google.com/dataplex/docs/fully-qualified-names.
The maximum size of the field is 4000 characters.</rdfs:comment>
    <rdfs:domain rdf:resource="http://example.org/onto/class/google_dataplex_entry"/>
    <rdfs:range rdf:resource="http://www.w3.org/2001/XMLSchema#string"/>
  </owl:DatatypeProperty>
  <owl:DatatypeProperty rdf:about="http://example.org/onto/prop/google_dataplex_entry_id">
    <rdfs:label>id</rdfs:label>
    <rdfs:domain rdf:resource="http://example.org/onto/class/google_dataplex_entry"/>
    <rdfs:range rdf:resource="http://www.w3.org/2001/XMLSchema#string"/>
  </owl:DatatypeProperty>
  <owl:DatatypeProperty rdf:about="http://example.org/onto/prop/google_dataplex_entry_location">
    <rdfs:label>location</rdfs:label>
    <rdfs:comment>The location where entry will be created.</rdfs:comment>
    <rdfs:domain rdf:resource="http://example.org/onto/class/google_dataplex_entry"/>
    <rdfs:range rdf:resource="http://www.w3.org/2001/XMLSchema#string"/>
  </owl:DatatypeProperty>
  <owl:DatatypeProperty rdf:about="http://example.org/onto/prop/google_dataplex_entry_name">
    <rdfs:label>name</rdfs:label>
    <rdfs:comment>The relative resource name of the entry, in the format projects/{project_number}/locations/{locationId}/entryGroups/{entryGroupId}/entries/{entryId}.</rdfs:comment>
    <rdfs:domain rdf:resource="http://example.org/onto/class/google_dataplex_entry"/>
    <rdfs:range rdf:resource="http://www.w3.org/2001/XMLSchema#string"/>
  </owl:DatatypeProperty>
  <owl:DatatypeProperty rdf:about="http://example.org/onto/prop/google_dataplex_entry_parent_entry">
    <rdfs:label>parent_entry</rdfs:label>
    <rdfs:comment>The resource name of the parent entry, in the format projects/{project_number}/locations/{locationId}/entryGroups/{entryGroupId}/entries/{entryId}.</rdfs:comment>
    <rdfs:domain rdf:resource="http://example.org/onto/class/google_dataplex_entry"/>
    <rdfs:range rdf:resource="http://www.w3.org/2001/XMLSchema#string"/>
  </owl:DatatypeProperty>
  <owl:DatatypeProperty rdf:about="http://example.org/onto/prop/google_dataplex_entry_project">
    <rdfs:label>project</rdfs:label>
    <rdfs:domain rdf:resource="http://example.org/onto/class/google_dataplex_entry"/>
    <rdfs:range rdf:resource="http://www.w3.org/2001/XMLSchema#string"/>
  </owl:DatatypeProperty>
  <owl:DatatypeProperty rdf:about="http://example.org/onto/prop/google_dataplex_entry_update_time">
    <rdfs:label>update_time</rdfs:label>
    <rdfs:comment>The time when the entry was last updated in Dataplex.</rdfs:comment>
    <rdfs:domain rdf:resource="http://example.org/onto/class/google_dataplex_entry"/>
    <rdfs:range rdf:resource="http://www.w3.org/2001/XMLSchema#string"/>
  </owl:DatatypeProperty>
  <owl:DatatypeProperty rdf:about="http://example.org/onto/prop/google_dataplex_entry_aspect_key">
    <rdfs:label>aspect_key</rdfs:label>
    <rdfs:comment>Depending on how the aspect is attached to the entry, the format of the aspect key can be one of the following:

If the aspect is attached directly to the entry: {project_number}.{locationId}.{aspectTypeId}
If the aspect is attached to an entry's path: {project_number}.{locationId}.{aspectTypeId}@{path}</rdfs:comment>
    <rdfs:domain rdf:resource="http://example.org/onto/class/google_dataplex_entry"/>
    <rdfs:range rdf:resource="http://www.w3.org/2001/XMLSchema#string"/>
  </owl:DatatypeProperty>
  <owl:DatatypeProperty rdf:about="http://example.org/onto/prop/google_dataplex_entry_aspect_type">
    <rdfs:label>aspect_type</rdfs:label>
    <rdfs:comment>The resource name of the type used to create this Aspect.</rdfs:comment>
    <rdfs:domain rdf:resource="http://example.org/onto/class/google_dataplex_entry"/>
    <rdfs:range rdf:resource="http://www.w3.org/2001/XMLSchema#string"/>
  </owl:DatatypeProperty>
  <owl:DatatypeProperty rdf:about="http://example.org/onto/prop/google_dataplex_entry_create_time">
    <rdfs:label>create_time</rdfs:label>
    <rdfs:comment>The time when the Aspect was created.</rdfs:comment>
    <rdfs:domain rdf:resource="http://example.org/onto/class/google_dataplex_entry"/>
    <rdfs:range rdf:resource="http://www.w3.org/2001/XMLSchema#string"/>
  </owl:DatatypeProperty>
  <owl:DatatypeProperty rdf:about="http://example.org/onto/prop/google_dataplex_entry_data">
    <rdfs:label>data</rdfs:label>
    <rdfs:comment>The content of the aspect in JSON form, according to its aspect type schema. The maximum size of the field is 120KB (encoded as UTF-8).</rdfs:comment>
    <rdfs:domain rdf:resource="http://example.org/onto/class/google_dataplex_entry"/>
    <rdfs:range rdf:resource="http://www.w3.org/2001/XMLSchema#string"/>
  </owl:DatatypeProperty>
  <owl:DatatypeProperty rdf:about="http://example.org/onto/prop/google_dataplex_entry_path">
    <rdfs:label>path</rdfs:label>
    <rdfs:comment>The path in the entry under which the aspect is attached.</rdfs:comment>
    <rdfs:domain rdf:resource="http://example.org/onto/class/google_dataplex_entry"/>
    <rdfs:range rdf:resource="http://www.w3.org/2001/XMLSchema#string"/>
  </owl:DatatypeProperty>
  <owl:DatatypeProperty rdf:about="http://example.org/onto/prop/google_dataplex_entry_update_time">
    <rdfs:label>update_time</rdfs:label>
    <rdfs:comment>The time when the Aspect was last modified.</rdfs:comment>
    <rdfs:domain rdf:resource="http://example.org/onto/class/google_dataplex_entry"/>
    <rdfs:range rdf:resource="http://www.w3.org/2001/XMLSchema#string"/>
  </owl:DatatypeProperty>
  <owl:DatatypeProperty rdf:about="http://example.org/onto/prop/google_dataplex_entry_create_time">
    <rdfs:label>create_time</rdfs:label>
    <rdfs:comment>The time when the resource was created in the source system.</rdfs:comment>
    <rdfs:domain rdf:resource="http://example.org/onto/class/google_dataplex_entry"/>
    <rdfs:range rdf:resource="http://www.w3.org/2001/XMLSchema#string"/>
  </owl:DatatypeProperty>
  <owl:DatatypeProperty rdf:about="http://example.org/onto/prop/google_dataplex_entry_description">
    <rdfs:label>description</rdfs:label>
    <rdfs:comment>A description of the data resource. Maximum length is 2,000 characters.</rdfs:comment>
    <rdfs:domain rdf:resource="http://example.org/onto/class/google_dataplex_entry"/>
    <rdfs:range rdf:resource="http://www.w3.org/2001/XMLSchema#string"/>
  </owl:DatatypeProperty>
  <owl:DatatypeProperty rdf:about="http://example.org/onto/prop/google_dataplex_entry_display_name">
    <rdfs:label>display_name</rdfs:label>
    <rdfs:comment>A user-friendly display name. Maximum length is 500 characters.</rdfs:comment>
    <rdfs:domain rdf:resource="http://example.org/onto/class/google_dataplex_entry"/>
    <rdfs:range rdf:resource="http://www.w3.org/2001/XMLSchema#string"/>
  </owl:DatatypeProperty>
  <owl:DatatypeProperty rdf:about="http://example.org/onto/prop/google_dataplex_entry_labels">
    <rdfs:label>labels</rdfs:label>
    <rdfs:comment>User-defined labels. The maximum size of keys and values is 128 characters each.
An object containing a list of "key": value pairs. Example: { "name": "wrench", "mass": "1.3kg", "count": "3" }.</rdfs:comment>
    <rdfs:domain rdf:resource="http://example.org/onto/class/google_dataplex_entry"/>
    <rdfs:range rdf:resource="http://www.w3.org/2001/XMLSchema#string"/>
  </owl:DatatypeProperty>
  <owl:DatatypeProperty rdf:about="http://example.org/onto/prop/google_dataplex_entry_location">
    <rdfs:label>location</rdfs:label>
    <rdfs:comment>Location of the resource in the source system. You can search the entry by this location.
By default, this should match the location of the entry group containing this entry.
A different value allows capturing the source location for data external to Google Cloud.</rdfs:comment>
    <rdfs:domain rdf:resource="http://example.org/onto/class/google_dataplex_entry"/>
    <rdfs:range rdf:resource="http://www.w3.org/2001/XMLSchema#string"/>
  </owl:DatatypeProperty>
  <owl:DatatypeProperty rdf:about="http://example.org/onto/prop/google_dataplex_entry_platform">
    <rdfs:label>platform</rdfs:label>
    <rdfs:comment>The platform containing the source system. Maximum length is 64 characters.</rdfs:comment>
    <rdfs:domain rdf:resource="http://example.org/onto/class/google_dataplex_entry"/>
    <rdfs:range rdf:resource="http://www.w3.org/2001/XMLSchema#string"/>
  </owl:DatatypeProperty>
  <owl:DatatypeProperty rdf:about="http://example.org/onto/prop/google_dataplex_entry_resource">
    <rdfs:label>resource</rdfs:label>
    <rdfs:comment>The name of the resource in the source system. Maximum length is 4,000 characters.</rdfs:comment>
    <rdfs:domain rdf:resource="http://example.org/onto/class/google_dataplex_entry"/>
    <rdfs:range rdf:resource="http://www.w3.org/2001/XMLSchema#string"/>
  </owl:DatatypeProperty>
  <owl:DatatypeProperty rdf:about="http://example.org/onto/prop/google_dataplex_entry_system">
    <rdfs:label>system</rdfs:label>
    <rdfs:comment>The name of the source system. Maximum length is 64 characters.</rdfs:comment>
    <rdfs:domain rdf:resource="http://example.org/onto/class/google_dataplex_entry"/>
    <rdfs:range rdf:resource="http://www.w3.org/2001/XMLSchema#string"/>
  </owl:DatatypeProperty>
  <owl:DatatypeProperty rdf:about="http://example.org/onto/prop/google_dataplex_entry_update_time">
    <rdfs:label>update_time</rdfs:label>
    <rdfs:comment>The time when the resource was last updated in the source system.
If the entry exists in the system and its EntrySource has updateTime populated,
further updates to the EntrySource of the entry must provide incremental updates to its updateTime.</rdfs:comment>
    <rdfs:domain rdf:resource="http://example.org/onto/class/google_dataplex_entry"/>
    <rdfs:range rdf:resource="http://www.w3.org/2001/XMLSchema#string"/>
  </owl:DatatypeProperty>
  <owl:DatatypeProperty rdf:about="http://example.org/onto/prop/google_dataplex_entry_name">
    <rdfs:label>name</rdfs:label>
    <rdfs:comment>The name of the ancestor resource.</rdfs:comment>
    <rdfs:domain rdf:resource="http://example.org/onto/class/google_dataplex_entry"/>
    <rdfs:range rdf:resource="http://www.w3.org/2001/XMLSchema#string"/>
  </owl:DatatypeProperty>
  <owl:DatatypeProperty rdf:about="http://example.org/onto/prop/google_dataplex_entry_type">
    <rdfs:label>type</rdfs:label>
    <rdfs:comment>The type of the ancestor resource.</rdfs:comment>
    <rdfs:domain rdf:resource="http://example.org/onto/class/google_dataplex_entry"/>
    <rdfs:range rdf:resource="http://www.w3.org/2001/XMLSchema#string"/>
  </owl:DatatypeProperty>
  <owl:DatatypeProperty rdf:about="http://example.org/onto/prop/google_dataplex_entry_create">
    <rdfs:label>create</rdfs:label>
    <rdfs:domain rdf:resource="http://example.org/onto/class/google_dataplex_entry"/>
    <rdfs:range rdf:resource="http://www.w3.org/2001/XMLSchema#string"/>
  </owl:DatatypeProperty>
  <owl:DatatypeProperty rdf:about="http://example.org/onto/prop/google_dataplex_entry_delete">
    <rdfs:label>delete</rdfs:label>
    <rdfs:domain rdf:resource="http://example.org/onto/class/google_dataplex_entry"/>
    <rdfs:range rdf:resource="http://www.w3.org/2001/XMLSchema#string"/>
  </owl:DatatypeProperty>
  <owl:DatatypeProperty rdf:about="http://example.org/onto/prop/google_dataplex_entry_update">
    <rdfs:label>update</rdfs:label>
    <rdfs:domain rdf:resource="http://example.org/onto/class/google_dataplex_entry"/>
    <rdfs:range rdf:resource="http://www.w3.org/2001/XMLSchema#string"/>
  </owl:DatatypeProperty>
</rdf:RDF>
