<?xml version="1.0" encoding="UTF-8"?>
<rdf:RDF
  xmlns:rdf="http://www.w3.org/1999/02/22-rdf-syntax-ns#"
  xmlns:rdfs="http://www.w3.org/2000/01/rdf-schema#"
  xmlns:owl="http://www.w3.org/2002/07/owl#"
  xmlns:xsd="http://www.w3.org/2001/XMLSchema#"
  xml:base="http://example.org/onto/">
  <owl:Class rdf:about="http://example.org/onto/class/google_container_aws_cluster">
    <rdfs:label>google_container_aws_cluster</rdfs:label>
    <rdfs:comment>#
#     ***     AUTO GENERATED CODE    ***    Type: DCL     ***
#
# ----------------------------------------------------------------------------
#
#     This file is managed by Magic Modules (https:#github.com/GoogleCloudPlatform/magic-modules)
#     and is based on the DCL (https:#github.com/GoogleCloudPlatform/declarative-resource-client-library).
#     Changes will need to be made to the DCL or Magic Modules instead of here.
#
#     We are not currently able to accept contributions to this file. If changes
#     are required, please file an issue at https:#github.com/hashicorp/terraform-provider-google/issues/new/choose
#
# ----------------------------------------------------------------------------
subcategory: "ContainerAws"
description: |-
  An Anthos cluster running on AWS.
---</rdfs:comment>
  </owl:Class>
  <owl:DatatypeProperty rdf:about="http://example.org/onto/prop/google_container_aws_cluster_annotations">
    <rdfs:label>annotations</rdfs:label>
    <rdfs:comment>Optional. Annotations on the cluster. This field has the same restrictions as Kubernetes annotations. The total size of all keys and values combined is limited to 256k. Key can have 2 segments: prefix (optional) and name (required), separated by a slash (/). Prefix must be a DNS subdomain. Name must be 63 characters or less, begin and end with alphanumerics, with dashes (-), underscores (_), dots (.), and alphanumerics between.

**Note**: This field is non-authoritative, and will only manage the annotations present in your configuration.
Please refer to the field `effective_annotations` for all of the annotations present on the resource.</rdfs:comment>
    <rdfs:domain rdf:resource="http://example.org/onto/class/google_container_aws_cluster"/>
    <rdfs:range rdf:resource="http://www.w3.org/2001/XMLSchema#string"/>
  </owl:DatatypeProperty>
  <owl:DatatypeProperty rdf:about="http://example.org/onto/prop/google_container_aws_cluster_aws_region">
    <rdfs:label>aws_region</rdfs:label>
    <rdfs:comment>The AWS region where the cluster runs. Each Google Cloud region supports a subset of nearby AWS regions. You can call to list all supported AWS regions within a given Google Cloud region.</rdfs:comment>
    <rdfs:domain rdf:resource="http://example.org/onto/class/google_container_aws_cluster"/>
    <rdfs:range rdf:resource="http://www.w3.org/2001/XMLSchema#string"/>
  </owl:DatatypeProperty>
  <owl:DatatypeProperty rdf:about="http://example.org/onto/prop/google_container_aws_cluster_create_time">
    <rdfs:label>create_time</rdfs:label>
    <rdfs:comment>Output only. The time at which this cluster was created.</rdfs:comment>
    <rdfs:domain rdf:resource="http://example.org/onto/class/google_container_aws_cluster"/>
    <rdfs:range rdf:resource="http://www.w3.org/2001/XMLSchema#string"/>
  </owl:DatatypeProperty>
  <owl:DatatypeProperty rdf:about="http://example.org/onto/prop/google_container_aws_cluster_description">
    <rdfs:label>description</rdfs:label>
    <rdfs:comment>Optional. A human readable description of this cluster. Cannot be longer than 255 UTF-8 encoded bytes.</rdfs:comment>
    <rdfs:domain rdf:resource="http://example.org/onto/class/google_container_aws_cluster"/>
    <rdfs:range rdf:resource="http://www.w3.org/2001/XMLSchema#string"/>
  </owl:DatatypeProperty>
  <owl:DatatypeProperty rdf:about="http://example.org/onto/prop/google_container_aws_cluster_effective_annotations">
    <rdfs:label>effective_annotations</rdfs:label>
    <rdfs:comment>All of annotations (key/value pairs) present on the resource in GCP, including the annotations configured through Terraform, other clients and services.</rdfs:comment>
    <rdfs:domain rdf:resource="http://example.org/onto/class/google_container_aws_cluster"/>
    <rdfs:range rdf:resource="http://www.w3.org/2001/XMLSchema#string"/>
  </owl:DatatypeProperty>
  <owl:DatatypeProperty rdf:about="http://example.org/onto/prop/google_container_aws_cluster_endpoint">
    <rdfs:label>endpoint</rdfs:label>
    <rdfs:comment>Output only. The endpoint of the cluster's API server.</rdfs:comment>
    <rdfs:domain rdf:resource="http://example.org/onto/class/google_container_aws_cluster"/>
    <rdfs:range rdf:resource="http://www.w3.org/2001/XMLSchema#string"/>
  </owl:DatatypeProperty>
  <owl:DatatypeProperty rdf:about="http://example.org/onto/prop/google_container_aws_cluster_etag">
    <rdfs:label>etag</rdfs:label>
    <rdfs:comment>Allows clients to perform consistent read-modify-writes through optimistic concurrency control. May be sent on update and delete requests to ensure the client has an up-to-date value before proceeding.</rdfs:comment>
    <rdfs:domain rdf:resource="http://example.org/onto/class/google_container_aws_cluster"/>
    <rdfs:range rdf:resource="http://www.w3.org/2001/XMLSchema#string"/>
  </owl:DatatypeProperty>
  <owl:DatatypeProperty rdf:about="http://example.org/onto/prop/google_container_aws_cluster_id">
    <rdfs:label>id</rdfs:label>
    <rdfs:domain rdf:resource="http://example.org/onto/class/google_container_aws_cluster"/>
    <rdfs:range rdf:resource="http://www.w3.org/2001/XMLSchema#string"/>
  </owl:DatatypeProperty>
  <owl:DatatypeProperty rdf:about="http://example.org/onto/prop/google_container_aws_cluster_location">
    <rdfs:label>location</rdfs:label>
    <rdfs:comment>The location for the resource</rdfs:comment>
    <rdfs:domain rdf:resource="http://example.org/onto/class/google_container_aws_cluster"/>
    <rdfs:range rdf:resource="http://www.w3.org/2001/XMLSchema#string"/>
  </owl:DatatypeProperty>
  <owl:DatatypeProperty rdf:about="http://example.org/onto/prop/google_container_aws_cluster_name">
    <rdfs:label>name</rdfs:label>
    <rdfs:comment>The name of this resource.</rdfs:comment>
    <rdfs:domain rdf:resource="http://example.org/onto/class/google_container_aws_cluster"/>
    <rdfs:range rdf:resource="http://www.w3.org/2001/XMLSchema#string"/>
  </owl:DatatypeProperty>
  <owl:DatatypeProperty rdf:about="http://example.org/onto/prop/google_container_aws_cluster_project">
    <rdfs:label>project</rdfs:label>
    <rdfs:comment>The project for the resource</rdfs:comment>
    <rdfs:domain rdf:resource="http://example.org/onto/class/google_container_aws_cluster"/>
    <rdfs:range rdf:resource="http://www.w3.org/2001/XMLSchema#string"/>
  </owl:DatatypeProperty>
  <owl:DatatypeProperty rdf:about="http://example.org/onto/prop/google_container_aws_cluster_reconciling">
    <rdfs:label>reconciling</rdfs:label>
    <rdfs:comment>Output only. If set, there are currently changes in flight to the cluster.</rdfs:comment>
    <rdfs:domain rdf:resource="http://example.org/onto/class/google_container_aws_cluster"/>
    <rdfs:range rdf:resource="http://www.w3.org/2001/XMLSchema#string"/>
  </owl:DatatypeProperty>
  <owl:DatatypeProperty rdf:about="http://example.org/onto/prop/google_container_aws_cluster_state">
    <rdfs:label>state</rdfs:label>
    <rdfs:comment>Output only. The current state of the cluster. Possible values: STATE_UNSPECIFIED, PROVISIONING, RUNNING, RECONCILING, STOPPING, ERROR, DEGRADED</rdfs:comment>
    <rdfs:domain rdf:resource="http://example.org/onto/class/google_container_aws_cluster"/>
    <rdfs:range rdf:resource="http://www.w3.org/2001/XMLSchema#string"/>
  </owl:DatatypeProperty>
  <owl:DatatypeProperty rdf:about="http://example.org/onto/prop/google_container_aws_cluster_uid">
    <rdfs:label>uid</rdfs:label>
    <rdfs:comment>Output only. A globally unique identifier for the cluster.</rdfs:comment>
    <rdfs:domain rdf:resource="http://example.org/onto/class/google_container_aws_cluster"/>
    <rdfs:range rdf:resource="http://www.w3.org/2001/XMLSchema#string"/>
  </owl:DatatypeProperty>
  <owl:DatatypeProperty rdf:about="http://example.org/onto/prop/google_container_aws_cluster_update_time">
    <rdfs:label>update_time</rdfs:label>
    <rdfs:comment>Output only. The time at which this cluster was last updated.</rdfs:comment>
    <rdfs:domain rdf:resource="http://example.org/onto/class/google_container_aws_cluster"/>
    <rdfs:range rdf:resource="http://www.w3.org/2001/XMLSchema#string"/>
  </owl:DatatypeProperty>
  <owl:DatatypeProperty rdf:about="http://example.org/onto/prop/google_container_aws_cluster_workload_identity_config">
    <rdfs:label>workload_identity_config</rdfs:label>
    <rdfs:comment>Output only. Workload Identity settings.</rdfs:comment>
    <rdfs:domain rdf:resource="http://example.org/onto/class/google_container_aws_cluster"/>
    <rdfs:range rdf:resource="http://www.w3.org/2001/XMLSchema#string"/>
  </owl:DatatypeProperty>
  <owl:DatatypeProperty rdf:about="http://example.org/onto/prop/google_container_aws_cluster_group">
    <rdfs:label>group</rdfs:label>
    <rdfs:comment>The name of the group, e.g. `my-group@domain.com`.</rdfs:comment>
    <rdfs:domain rdf:resource="http://example.org/onto/class/google_container_aws_cluster"/>
    <rdfs:range rdf:resource="http://www.w3.org/2001/XMLSchema#string"/>
  </owl:DatatypeProperty>
  <owl:DatatypeProperty rdf:about="http://example.org/onto/prop/google_container_aws_cluster_username">
    <rdfs:label>username</rdfs:label>
    <rdfs:comment>The name of the user, e.g. `my-gcp-id@gmail.com`.</rdfs:comment>
    <rdfs:domain rdf:resource="http://example.org/onto/class/google_container_aws_cluster"/>
    <rdfs:range rdf:resource="http://www.w3.org/2001/XMLSchema#string"/>
  </owl:DatatypeProperty>
  <owl:DatatypeProperty rdf:about="http://example.org/onto/prop/google_container_aws_cluster_evaluation_mode">
    <rdfs:label>evaluation_mode</rdfs:label>
    <rdfs:comment>Mode of operation for Binary Authorization policy evaluation. Possible values: DISABLED, PROJECT_SINGLETON_POLICY_ENFORCE</rdfs:comment>
    <rdfs:domain rdf:resource="http://example.org/onto/class/google_container_aws_cluster"/>
    <rdfs:range rdf:resource="http://www.w3.org/2001/XMLSchema#string"/>
  </owl:DatatypeProperty>
  <owl:DatatypeProperty rdf:about="http://example.org/onto/prop/google_container_aws_cluster_iam_instance_profile">
    <rdfs:label>iam_instance_profile</rdfs:label>
    <rdfs:comment>The name of the AWS IAM instance pofile to assign to each control plane replica.</rdfs:comment>
    <rdfs:domain rdf:resource="http://example.org/onto/class/google_container_aws_cluster"/>
    <rdfs:range rdf:resource="http://www.w3.org/2001/XMLSchema#string"/>
  </owl:DatatypeProperty>
  <owl:DatatypeProperty rdf:about="http://example.org/onto/prop/google_container_aws_cluster_instance_type">
    <rdfs:label>instance_type</rdfs:label>
    <rdfs:comment>Optional. The AWS instance type. When unspecified, it defaults to `m5.large`.</rdfs:comment>
    <rdfs:domain rdf:resource="http://example.org/onto/class/google_container_aws_cluster"/>
    <rdfs:range rdf:resource="http://www.w3.org/2001/XMLSchema#string"/>
  </owl:DatatypeProperty>
  <owl:DatatypeProperty rdf:about="http://example.org/onto/prop/google_container_aws_cluster_security_group_ids">
    <rdfs:label>security_group_ids</rdfs:label>
    <rdfs:comment>Optional. The IDs of additional security groups to add to control plane replicas. The Anthos Multi-Cloud API will automatically create and manage security groups with the minimum rules needed for a functioning cluster.</rdfs:comment>
    <rdfs:domain rdf:resource="http://example.org/onto/class/google_container_aws_cluster"/>
    <rdfs:range rdf:resource="http://www.w3.org/2001/XMLSchema#string"/>
  </owl:DatatypeProperty>
  <owl:DatatypeProperty rdf:about="http://example.org/onto/prop/google_container_aws_cluster_subnet_ids">
    <rdfs:label>subnet_ids</rdfs:label>
    <rdfs:comment>The list of subnets where control plane replicas will run. A replica will be provisioned on each subnet and up to three values can be provided. Each subnet must be in a different AWS Availability Zone (AZ).</rdfs:comment>
    <rdfs:domain rdf:resource="http://example.org/onto/class/google_container_aws_cluster"/>
    <rdfs:range rdf:resource="http://www.w3.org/2001/XMLSchema#string"/>
  </owl:DatatypeProperty>
  <owl:DatatypeProperty rdf:about="http://example.org/onto/prop/google_container_aws_cluster_tags">
    <rdfs:label>tags</rdfs:label>
    <rdfs:comment>Optional. A set of AWS resource tags to propagate to all underlying managed AWS resources. Specify at most 50 pairs containing alphanumerics, spaces, and symbols (.+-=_:@/). Keys can be up to 127 Unicode characters. Values can be up to 255 Unicode characters.</rdfs:comment>
    <rdfs:domain rdf:resource="http://example.org/onto/class/google_container_aws_cluster"/>
    <rdfs:range rdf:resource="http://www.w3.org/2001/XMLSchema#string"/>
  </owl:DatatypeProperty>
  <owl:DatatypeProperty rdf:about="http://example.org/onto/prop/google_container_aws_cluster_version">
    <rdfs:label>version</rdfs:label>
    <rdfs:comment>The Kubernetes version to run on control plane replicas (e.g. `1.19.10-gke.1000`). You can list all supported versions on a given Google Cloud region by calling .</rdfs:comment>
    <rdfs:domain rdf:resource="http://example.org/onto/class/google_container_aws_cluster"/>
    <rdfs:range rdf:resource="http://www.w3.org/2001/XMLSchema#string"/>
  </owl:DatatypeProperty>
  <owl:DatatypeProperty rdf:about="http://example.org/onto/prop/google_container_aws_cluster_role_arn">
    <rdfs:label>role_arn</rdfs:label>
    <rdfs:comment>The Amazon Resource Name (ARN) of the role that the Anthos Multi-Cloud API will assume when managing AWS resources on your account.</rdfs:comment>
    <rdfs:domain rdf:resource="http://example.org/onto/class/google_container_aws_cluster"/>
    <rdfs:range rdf:resource="http://www.w3.org/2001/XMLSchema#string"/>
  </owl:DatatypeProperty>
  <owl:DatatypeProperty rdf:about="http://example.org/onto/prop/google_container_aws_cluster_role_session_name">
    <rdfs:label>role_session_name</rdfs:label>
    <rdfs:comment>Optional. An identifier for the assumed role session. When unspecified, it defaults to `multicloud-service-agent`.</rdfs:comment>
    <rdfs:domain rdf:resource="http://example.org/onto/class/google_container_aws_cluster"/>
    <rdfs:range rdf:resource="http://www.w3.org/2001/XMLSchema#string"/>
  </owl:DatatypeProperty>
  <owl:DatatypeProperty rdf:about="http://example.org/onto/prop/google_container_aws_cluster_kms_key_arn">
    <rdfs:label>kms_key_arn</rdfs:label>
    <rdfs:comment>The ARN of the AWS KMS key used to encrypt cluster configuration.</rdfs:comment>
    <rdfs:domain rdf:resource="http://example.org/onto/class/google_container_aws_cluster"/>
    <rdfs:range rdf:resource="http://www.w3.org/2001/XMLSchema#string"/>
  </owl:DatatypeProperty>
  <owl:DatatypeProperty rdf:about="http://example.org/onto/prop/google_container_aws_cluster_kms_key_arn">
    <rdfs:label>kms_key_arn</rdfs:label>
    <rdfs:comment>The ARN of the AWS KMS key used to encrypt cluster secrets.</rdfs:comment>
    <rdfs:domain rdf:resource="http://example.org/onto/class/google_container_aws_cluster"/>
    <rdfs:range rdf:resource="http://www.w3.org/2001/XMLSchema#string"/>
  </owl:DatatypeProperty>
  <owl:DatatypeProperty rdf:about="http://example.org/onto/prop/google_container_aws_cluster_iops">
    <rdfs:label>iops</rdfs:label>
    <rdfs:comment>Optional. The number of I/O operations per second (IOPS) to provision for GP3 volume.</rdfs:comment>
    <rdfs:domain rdf:resource="http://example.org/onto/class/google_container_aws_cluster"/>
    <rdfs:range rdf:resource="http://www.w3.org/2001/XMLSchema#string"/>
  </owl:DatatypeProperty>
  <owl:DatatypeProperty rdf:about="http://example.org/onto/prop/google_container_aws_cluster_kms_key_arn">
    <rdfs:label>kms_key_arn</rdfs:label>
    <rdfs:comment>Optional. The Amazon Resource Name (ARN) of the Customer Managed Key (CMK) used to encrypt AWS EBS volumes. If not specified, the default Amazon managed key associated to the AWS region where this cluster runs will be used.</rdfs:comment>
    <rdfs:domain rdf:resource="http://example.org/onto/class/google_container_aws_cluster"/>
    <rdfs:range rdf:resource="http://www.w3.org/2001/XMLSchema#string"/>
  </owl:DatatypeProperty>
  <owl:DatatypeProperty rdf:about="http://example.org/onto/prop/google_container_aws_cluster_size_gib">
    <rdfs:label>size_gib</rdfs:label>
    <rdfs:comment>Optional. The size of the volume, in GiBs. When unspecified, a default value is provided. See the specific reference in the parent resource.</rdfs:comment>
    <rdfs:domain rdf:resource="http://example.org/onto/class/google_container_aws_cluster"/>
    <rdfs:range rdf:resource="http://www.w3.org/2001/XMLSchema#string"/>
  </owl:DatatypeProperty>
  <owl:DatatypeProperty rdf:about="http://example.org/onto/prop/google_container_aws_cluster_throughput">
    <rdfs:label>throughput</rdfs:label>
    <rdfs:comment>Optional. The throughput to provision for the volume, in MiB/s. Only valid if the volume type is GP3. If volume type is gp3 and throughput is not specified, the throughput will defaults to 125.</rdfs:comment>
    <rdfs:domain rdf:resource="http://example.org/onto/class/google_container_aws_cluster"/>
    <rdfs:range rdf:resource="http://www.w3.org/2001/XMLSchema#string"/>
  </owl:DatatypeProperty>
  <owl:DatatypeProperty rdf:about="http://example.org/onto/prop/google_container_aws_cluster_volume_type">
    <rdfs:label>volume_type</rdfs:label>
    <rdfs:comment>Optional. Type of the EBS volume. When unspecified, it defaults to GP2 volume. Possible values: VOLUME_TYPE_UNSPECIFIED, GP2, GP3</rdfs:comment>
    <rdfs:domain rdf:resource="http://example.org/onto/class/google_container_aws_cluster"/>
    <rdfs:range rdf:resource="http://www.w3.org/2001/XMLSchema#string"/>
  </owl:DatatypeProperty>
  <owl:DatatypeProperty rdf:about="http://example.org/onto/prop/google_container_aws_cluster_secret_arn">
    <rdfs:label>secret_arn</rdfs:label>
    <rdfs:comment>The ARN of the AWS Secret Manager secret that contains the HTTP(S) proxy configuration.</rdfs:comment>
    <rdfs:domain rdf:resource="http://example.org/onto/class/google_container_aws_cluster"/>
    <rdfs:range rdf:resource="http://www.w3.org/2001/XMLSchema#string"/>
  </owl:DatatypeProperty>
  <owl:DatatypeProperty rdf:about="http://example.org/onto/prop/google_container_aws_cluster_secret_version">
    <rdfs:label>secret_version</rdfs:label>
    <rdfs:comment>The version string of the AWS Secret Manager secret that contains the HTTP(S) proxy configuration.</rdfs:comment>
    <rdfs:domain rdf:resource="http://example.org/onto/class/google_container_aws_cluster"/>
    <rdfs:range rdf:resource="http://www.w3.org/2001/XMLSchema#string"/>
  </owl:DatatypeProperty>
  <owl:DatatypeProperty rdf:about="http://example.org/onto/prop/google_container_aws_cluster_iops">
    <rdfs:label>iops</rdfs:label>
    <rdfs:comment>Optional. The number of I/O operations per second (IOPS) to provision for GP3 volume.</rdfs:comment>
    <rdfs:domain rdf:resource="http://example.org/onto/class/google_container_aws_cluster"/>
    <rdfs:range rdf:resource="http://www.w3.org/2001/XMLSchema#string"/>
  </owl:DatatypeProperty>
  <owl:DatatypeProperty rdf:about="http://example.org/onto/prop/google_container_aws_cluster_kms_key_arn">
    <rdfs:label>kms_key_arn</rdfs:label>
    <rdfs:comment>Optional. The Amazon Resource Name (ARN) of the Customer Managed Key (CMK) used to encrypt AWS EBS volumes. If not specified, the default Amazon managed key associated to the AWS region where this cluster runs will be used.</rdfs:comment>
    <rdfs:domain rdf:resource="http://example.org/onto/class/google_container_aws_cluster"/>
    <rdfs:range rdf:resource="http://www.w3.org/2001/XMLSchema#string"/>
  </owl:DatatypeProperty>
  <owl:DatatypeProperty rdf:about="http://example.org/onto/prop/google_container_aws_cluster_size_gib">
    <rdfs:label>size_gib</rdfs:label>
    <rdfs:comment>Optional. The size of the volume, in GiBs. When unspecified, a default value is provided. See the specific reference in the parent resource.</rdfs:comment>
    <rdfs:domain rdf:resource="http://example.org/onto/class/google_container_aws_cluster"/>
    <rdfs:range rdf:resource="http://www.w3.org/2001/XMLSchema#string"/>
  </owl:DatatypeProperty>
  <owl:DatatypeProperty rdf:about="http://example.org/onto/prop/google_container_aws_cluster_throughput">
    <rdfs:label>throughput</rdfs:label>
    <rdfs:comment>Optional. The throughput to provision for the volume, in MiB/s. Only valid if the volume type is GP3. If volume type is gp3 and throughput is not specified, the throughput will defaults to 125.</rdfs:comment>
    <rdfs:domain rdf:resource="http://example.org/onto/class/google_container_aws_cluster"/>
    <rdfs:range rdf:resource="http://www.w3.org/2001/XMLSchema#string"/>
  </owl:DatatypeProperty>
  <owl:DatatypeProperty rdf:about="http://example.org/onto/prop/google_container_aws_cluster_volume_type">
    <rdfs:label>volume_type</rdfs:label>
    <rdfs:comment>Optional. Type of the EBS volume. When unspecified, it defaults to GP2 volume. Possible values: VOLUME_TYPE_UNSPECIFIED, GP2, GP3</rdfs:comment>
    <rdfs:domain rdf:resource="http://example.org/onto/class/google_container_aws_cluster"/>
    <rdfs:range rdf:resource="http://www.w3.org/2001/XMLSchema#string"/>
  </owl:DatatypeProperty>
  <owl:DatatypeProperty rdf:about="http://example.org/onto/prop/google_container_aws_cluster_ec2_key_pair">
    <rdfs:label>ec2_key_pair</rdfs:label>
    <rdfs:comment>The name of the EC2 key pair used to login into cluster machines.</rdfs:comment>
    <rdfs:domain rdf:resource="http://example.org/onto/class/google_container_aws_cluster"/>
    <rdfs:range rdf:resource="http://www.w3.org/2001/XMLSchema#string"/>
  </owl:DatatypeProperty>
  <owl:DatatypeProperty rdf:about="http://example.org/onto/prop/google_container_aws_cluster_membership">
    <rdfs:label>membership</rdfs:label>
    <rdfs:comment>The name of the managed Hub Membership resource associated to this cluster. Membership names are formatted as projects/<project-number>/locations/global/membership/<cluster-id>.</rdfs:comment>
    <rdfs:domain rdf:resource="http://example.org/onto/class/google_container_aws_cluster"/>
    <rdfs:range rdf:resource="http://www.w3.org/2001/XMLSchema#string"/>
  </owl:DatatypeProperty>
  <owl:DatatypeProperty rdf:about="http://example.org/onto/prop/google_container_aws_cluster_project">
    <rdfs:label>project</rdfs:label>
    <rdfs:comment>The number of the Fleet host project where this cluster will be registered.</rdfs:comment>
    <rdfs:domain rdf:resource="http://example.org/onto/class/google_container_aws_cluster"/>
    <rdfs:range rdf:resource="http://www.w3.org/2001/XMLSchema#string"/>
  </owl:DatatypeProperty>
  <owl:DatatypeProperty rdf:about="http://example.org/onto/prop/google_container_aws_cluster_per_node_pool_sg_rules_disabled">
    <rdfs:label>per_node_pool_sg_rules_disabled</rdfs:label>
    <rdfs:comment>Disable the per node pool subnet security group rules on the control plane security group. When set to true, you must also provide one or more security groups that ensure node pools are able to send requests to the control plane on TCP/443 and TCP/8132. Failure to do so may result in unavailable node pools.</rdfs:comment>
    <rdfs:domain rdf:resource="http://example.org/onto/class/google_container_aws_cluster"/>
    <rdfs:range rdf:resource="http://www.w3.org/2001/XMLSchema#string"/>
  </owl:DatatypeProperty>
  <owl:DatatypeProperty rdf:about="http://example.org/onto/prop/google_container_aws_cluster_pod_address_cidr_blocks">
    <rdfs:label>pod_address_cidr_blocks</rdfs:label>
    <rdfs:comment>All pods in the cluster are assigned an RFC1918 IPv4 address from these ranges. Only a single range is supported. This field cannot be changed after creation.</rdfs:comment>
    <rdfs:domain rdf:resource="http://example.org/onto/class/google_container_aws_cluster"/>
    <rdfs:range rdf:resource="http://www.w3.org/2001/XMLSchema#string"/>
  </owl:DatatypeProperty>
  <owl:DatatypeProperty rdf:about="http://example.org/onto/prop/google_container_aws_cluster_service_address_cidr_blocks">
    <rdfs:label>service_address_cidr_blocks</rdfs:label>
    <rdfs:comment>All services in the cluster are assigned an RFC1918 IPv4 address from these ranges. Only a single range is supported. This field cannot be changed after creation.</rdfs:comment>
    <rdfs:domain rdf:resource="http://example.org/onto/class/google_container_aws_cluster"/>
    <rdfs:range rdf:resource="http://www.w3.org/2001/XMLSchema#string"/>
  </owl:DatatypeProperty>
  <owl:DatatypeProperty rdf:about="http://example.org/onto/prop/google_container_aws_cluster_vpc_id">
    <rdfs:label>vpc_id</rdfs:label>
    <rdfs:comment>The VPC associated with the cluster. All component clusters (i.e. control plane and node pools) run on a single VPC. This field cannot be changed after creation.</rdfs:comment>
    <rdfs:domain rdf:resource="http://example.org/onto/class/google_container_aws_cluster"/>
    <rdfs:range rdf:resource="http://www.w3.org/2001/XMLSchema#string"/>
  </owl:DatatypeProperty>
  <owl:DatatypeProperty rdf:about="http://example.org/onto/prop/google_container_aws_cluster_create">
    <rdfs:label>create</rdfs:label>
    <rdfs:domain rdf:resource="http://example.org/onto/class/google_container_aws_cluster"/>
    <rdfs:range rdf:resource="http://www.w3.org/2001/XMLSchema#string"/>
  </owl:DatatypeProperty>
  <owl:DatatypeProperty rdf:about="http://example.org/onto/prop/google_container_aws_cluster_delete">
    <rdfs:label>delete</rdfs:label>
    <rdfs:domain rdf:resource="http://example.org/onto/class/google_container_aws_cluster"/>
    <rdfs:range rdf:resource="http://www.w3.org/2001/XMLSchema#string"/>
  </owl:DatatypeProperty>
  <owl:DatatypeProperty rdf:about="http://example.org/onto/prop/google_container_aws_cluster_update">
    <rdfs:label>update</rdfs:label>
    <rdfs:domain rdf:resource="http://example.org/onto/class/google_container_aws_cluster"/>
    <rdfs:range rdf:resource="http://www.w3.org/2001/XMLSchema#string"/>
  </owl:DatatypeProperty>
</rdf:RDF>
