<?xml version="1.0" encoding="UTF-8"?>
<rdf:RDF
  xmlns:rdf="http://www.w3.org/1999/02/22-rdf-syntax-ns#"
  xmlns:rdfs="http://www.w3.org/2000/01/rdf-schema#"
  xmlns:owl="http://www.w3.org/2002/07/owl#"
  xmlns:xsd="http://www.w3.org/2001/XMLSchema#"
  xml:base="http://example.org/onto/">
  <owl:Class rdf:about="http://example.org/onto/class/google_service_account">
    <rdfs:label>google_service_account</rdfs:label>
  </owl:Class>
  <owl:DatatypeProperty rdf:about="http://example.org/onto/prop/google_service_account_account_id">
    <rdfs:label>account_id</rdfs:label>
    <rdfs:comment>The account id that is used to generate the service account email address and a stable unique id. It is unique within a project, must be 6-30 characters long, and match the regular expression [a-z]([-a-z0-9]*[a-z0-9]) to comply with RFC1035. Changing this forces a new service account to be created.</rdfs:comment>
    <rdfs:domain rdf:resource="http://example.org/onto/class/google_service_account"/>
    <rdfs:range rdf:resource="http://www.w3.org/2001/XMLSchema#string"/>
  </owl:DatatypeProperty>
  <owl:DatatypeProperty rdf:about="http://example.org/onto/prop/google_service_account_create_ignore_already_exists">
    <rdfs:label>create_ignore_already_exists</rdfs:label>
    <rdfs:comment>If set to true, skip service account creation if a service account with the same email already exists.</rdfs:comment>
    <rdfs:domain rdf:resource="http://example.org/onto/class/google_service_account"/>
    <rdfs:range rdf:resource="http://www.w3.org/2001/XMLSchema#string"/>
  </owl:DatatypeProperty>
  <owl:DatatypeProperty rdf:about="http://example.org/onto/prop/google_service_account_description">
    <rdfs:label>description</rdfs:label>
    <rdfs:comment>A text description of the service account. Must be less than or equal to 256 UTF-8 bytes.</rdfs:comment>
    <rdfs:domain rdf:resource="http://example.org/onto/class/google_service_account"/>
    <rdfs:range rdf:resource="http://www.w3.org/2001/XMLSchema#string"/>
  </owl:DatatypeProperty>
  <owl:DatatypeProperty rdf:about="http://example.org/onto/prop/google_service_account_disabled">
    <rdfs:label>disabled</rdfs:label>
    <rdfs:comment>Whether the service account is disabled. Defaults to false</rdfs:comment>
    <rdfs:domain rdf:resource="http://example.org/onto/class/google_service_account"/>
    <rdfs:range rdf:resource="http://www.w3.org/2001/XMLSchema#string"/>
  </owl:DatatypeProperty>
  <owl:DatatypeProperty rdf:about="http://example.org/onto/prop/google_service_account_display_name">
    <rdfs:label>display_name</rdfs:label>
    <rdfs:comment>The display name for the service account. Can be updated without creating a new resource.</rdfs:comment>
    <rdfs:domain rdf:resource="http://example.org/onto/class/google_service_account"/>
    <rdfs:range rdf:resource="http://www.w3.org/2001/XMLSchema#string"/>
  </owl:DatatypeProperty>
  <owl:DatatypeProperty rdf:about="http://example.org/onto/prop/google_service_account_email">
    <rdfs:label>email</rdfs:label>
    <rdfs:comment>The e-mail address of the service account. This value should be referenced from any google_iam_policy data sources that would grant the service account privileges.</rdfs:comment>
    <rdfs:domain rdf:resource="http://example.org/onto/class/google_service_account"/>
    <rdfs:range rdf:resource="http://www.w3.org/2001/XMLSchema#string"/>
  </owl:DatatypeProperty>
  <owl:DatatypeProperty rdf:about="http://example.org/onto/prop/google_service_account_id">
    <rdfs:label>id</rdfs:label>
    <rdfs:domain rdf:resource="http://example.org/onto/class/google_service_account"/>
    <rdfs:range rdf:resource="http://www.w3.org/2001/XMLSchema#string"/>
  </owl:DatatypeProperty>
  <owl:DatatypeProperty rdf:about="http://example.org/onto/prop/google_service_account_member">
    <rdfs:label>member</rdfs:label>
    <rdfs:comment>The Identity of the service account in the form 'serviceAccount:{email}'. This value is often used to refer to the service account in order to grant IAM permissions.</rdfs:comment>
    <rdfs:domain rdf:resource="http://example.org/onto/class/google_service_account"/>
    <rdfs:range rdf:resource="http://www.w3.org/2001/XMLSchema#string"/>
  </owl:DatatypeProperty>
  <owl:DatatypeProperty rdf:about="http://example.org/onto/prop/google_service_account_name">
    <rdfs:label>name</rdfs:label>
    <rdfs:comment>The fully-qualified name of the service account.</rdfs:comment>
    <rdfs:domain rdf:resource="http://example.org/onto/class/google_service_account"/>
    <rdfs:range rdf:resource="http://www.w3.org/2001/XMLSchema#string"/>
  </owl:DatatypeProperty>
  <owl:DatatypeProperty rdf:about="http://example.org/onto/prop/google_service_account_project">
    <rdfs:label>project</rdfs:label>
    <rdfs:comment>The ID of the project that the service account will be created in. Defaults to the provider project configuration.</rdfs:comment>
    <rdfs:domain rdf:resource="http://example.org/onto/class/google_service_account"/>
    <rdfs:range rdf:resource="http://www.w3.org/2001/XMLSchema#string"/>
  </owl:DatatypeProperty>
  <owl:DatatypeProperty rdf:about="http://example.org/onto/prop/google_service_account_unique_id">
    <rdfs:label>unique_id</rdfs:label>
    <rdfs:comment>The unique id of the service account.</rdfs:comment>
    <rdfs:domain rdf:resource="http://example.org/onto/class/google_service_account"/>
    <rdfs:range rdf:resource="http://www.w3.org/2001/XMLSchema#string"/>
  </owl:DatatypeProperty>
  <owl:DatatypeProperty rdf:about="http://example.org/onto/prop/google_service_account_create">
    <rdfs:label>create</rdfs:label>
    <rdfs:domain rdf:resource="http://example.org/onto/class/google_service_account"/>
    <rdfs:range rdf:resource="http://www.w3.org/2001/XMLSchema#string"/>
  </owl:DatatypeProperty>
</rdf:RDF>
