<?xml version="1.0" encoding="UTF-8"?>
<rdf:RDF
  xmlns:rdf="http://www.w3.org/1999/02/22-rdf-syntax-ns#"
  xmlns:rdfs="http://www.w3.org/2000/01/rdf-schema#"
  xmlns:owl="http://www.w3.org/2002/07/owl#"
  xmlns:xsd="http://www.w3.org/2001/XMLSchema#"
  xml:base="http://example.org/onto/">
  <owl:Class rdf:about="http://example.org/onto/class/google_eventarc_enrollment">
    <rdfs:label>google_eventarc_enrollment</rdfs:label>
    <rdfs:comment>#
#     ***     AUTO GENERATED CODE    ***    Type: MMv1     ***
#
# ----------------------------------------------------------------------------
#
#     This code is generated by Magic Modules using the following:
#
#     Configuration: https:#github.com/GoogleCloudPlatform/magic-modules/tree/main/mmv1/products/eventarc/Enrollment.yaml
#     Template:      https:#github.com/GoogleCloudPlatform/magic-modules/tree/main/mmv1/templates/terraform/resource.html.markdown.tmpl
#
#     DO NOT EDIT this file directly. Any changes made to this file will be
#     overwritten during the next generation cycle.
#
# ----------------------------------------------------------------------------
subcategory: "Eventarc"
description: |-
  The Eventarc Enrollment resource
---</rdfs:comment>
  </owl:Class>
  <owl:DatatypeProperty rdf:about="http://example.org/onto/prop/google_eventarc_enrollment_annotations">
    <rdfs:label>annotations</rdfs:label>
    <rdfs:comment>Resource annotations.

**Note**: This field is non-authoritative, and will only manage the annotations present in your configuration.
Please refer to the field 'effective_annotations' for all of the annotations present on the resource.</rdfs:comment>
    <rdfs:domain rdf:resource="http://example.org/onto/class/google_eventarc_enrollment"/>
    <rdfs:range rdf:resource="http://www.w3.org/2001/XMLSchema#string"/>
  </owl:DatatypeProperty>
  <owl:DatatypeProperty rdf:about="http://example.org/onto/prop/google_eventarc_enrollment_cel_match">
    <rdfs:label>cel_match</rdfs:label>
    <rdfs:comment>A CEL expression identifying which messages this enrollment applies to.</rdfs:comment>
    <rdfs:domain rdf:resource="http://example.org/onto/class/google_eventarc_enrollment"/>
    <rdfs:range rdf:resource="http://www.w3.org/2001/XMLSchema#string"/>
  </owl:DatatypeProperty>
  <owl:DatatypeProperty rdf:about="http://example.org/onto/prop/google_eventarc_enrollment_create_time">
    <rdfs:label>create_time</rdfs:label>
    <rdfs:comment>The creation time.</rdfs:comment>
    <rdfs:domain rdf:resource="http://example.org/onto/class/google_eventarc_enrollment"/>
    <rdfs:range rdf:resource="http://www.w3.org/2001/XMLSchema#string"/>
  </owl:DatatypeProperty>
  <owl:DatatypeProperty rdf:about="http://example.org/onto/prop/google_eventarc_enrollment_destination">
    <rdfs:label>destination</rdfs:label>
    <rdfs:comment>Destination is the Pipeline that the Enrollment is delivering to. It must
point to the full resource name of a Pipeline. Format:
"projects/{PROJECT_ID}/locations/{region}/pipelines/{PIPELINE_ID)"</rdfs:comment>
    <rdfs:domain rdf:resource="http://example.org/onto/class/google_eventarc_enrollment"/>
    <rdfs:range rdf:resource="http://www.w3.org/2001/XMLSchema#string"/>
  </owl:DatatypeProperty>
  <owl:DatatypeProperty rdf:about="http://example.org/onto/prop/google_eventarc_enrollment_display_name">
    <rdfs:label>display_name</rdfs:label>
    <rdfs:comment>Resource display name.</rdfs:comment>
    <rdfs:domain rdf:resource="http://example.org/onto/class/google_eventarc_enrollment"/>
    <rdfs:range rdf:resource="http://www.w3.org/2001/XMLSchema#string"/>
  </owl:DatatypeProperty>
  <owl:DatatypeProperty rdf:about="http://example.org/onto/prop/google_eventarc_enrollment_effective_annotations">
    <rdfs:label>effective_annotations</rdfs:label>
    <rdfs:comment>All of annotations (key/value pairs) present on the resource in GCP, including the annotations configured through Terraform, other clients and services.</rdfs:comment>
    <rdfs:domain rdf:resource="http://example.org/onto/class/google_eventarc_enrollment"/>
    <rdfs:range rdf:resource="http://www.w3.org/2001/XMLSchema#string"/>
  </owl:DatatypeProperty>
  <owl:DatatypeProperty rdf:about="http://example.org/onto/prop/google_eventarc_enrollment_effective_labels">
    <rdfs:label>effective_labels</rdfs:label>
    <rdfs:comment>All of labels (key/value pairs) present on the resource in GCP, including the labels configured through Terraform, other clients and services.</rdfs:comment>
    <rdfs:domain rdf:resource="http://example.org/onto/class/google_eventarc_enrollment"/>
    <rdfs:range rdf:resource="http://www.w3.org/2001/XMLSchema#string"/>
  </owl:DatatypeProperty>
  <owl:DatatypeProperty rdf:about="http://example.org/onto/prop/google_eventarc_enrollment_enrollment_id">
    <rdfs:label>enrollment_id</rdfs:label>
    <rdfs:comment>The user-provided ID to be assigned to the Enrollment. It should match the
format '^[a-z]([a-z0-9-]{0,61}[a-z0-9])?$'.</rdfs:comment>
    <rdfs:domain rdf:resource="http://example.org/onto/class/google_eventarc_enrollment"/>
    <rdfs:range rdf:resource="http://www.w3.org/2001/XMLSchema#string"/>
  </owl:DatatypeProperty>
  <owl:DatatypeProperty rdf:about="http://example.org/onto/prop/google_eventarc_enrollment_etag">
    <rdfs:label>etag</rdfs:label>
    <rdfs:comment>This checksum is computed by the server based on the value of other
fields, and might be sent only on update and delete requests to ensure that
the client has an up-to-date value before proceeding.</rdfs:comment>
    <rdfs:domain rdf:resource="http://example.org/onto/class/google_eventarc_enrollment"/>
    <rdfs:range rdf:resource="http://www.w3.org/2001/XMLSchema#string"/>
  </owl:DatatypeProperty>
  <owl:DatatypeProperty rdf:about="http://example.org/onto/prop/google_eventarc_enrollment_id">
    <rdfs:label>id</rdfs:label>
    <rdfs:domain rdf:resource="http://example.org/onto/class/google_eventarc_enrollment"/>
    <rdfs:range rdf:resource="http://www.w3.org/2001/XMLSchema#string"/>
  </owl:DatatypeProperty>
  <owl:DatatypeProperty rdf:about="http://example.org/onto/prop/google_eventarc_enrollment_labels">
    <rdfs:label>labels</rdfs:label>
    <rdfs:comment>Resource labels.

**Note**: This field is non-authoritative, and will only manage the labels present in your configuration.
Please refer to the field 'effective_labels' for all of the labels present on the resource.</rdfs:comment>
    <rdfs:domain rdf:resource="http://example.org/onto/class/google_eventarc_enrollment"/>
    <rdfs:range rdf:resource="http://www.w3.org/2001/XMLSchema#string"/>
  </owl:DatatypeProperty>
  <owl:DatatypeProperty rdf:about="http://example.org/onto/prop/google_eventarc_enrollment_location">
    <rdfs:label>location</rdfs:label>
    <rdfs:comment>Resource ID segment making up resource 'name'. It identifies the resource within its parent collection as described in https://google.aip.dev/122.</rdfs:comment>
    <rdfs:domain rdf:resource="http://example.org/onto/class/google_eventarc_enrollment"/>
    <rdfs:range rdf:resource="http://www.w3.org/2001/XMLSchema#string"/>
  </owl:DatatypeProperty>
  <owl:DatatypeProperty rdf:about="http://example.org/onto/prop/google_eventarc_enrollment_message_bus">
    <rdfs:label>message_bus</rdfs:label>
    <rdfs:comment>Resource name of the message bus identifying the source of the messages. It
matches the form
projects/{project}/locations/{location}/messageBuses/{messageBus}.</rdfs:comment>
    <rdfs:domain rdf:resource="http://example.org/onto/class/google_eventarc_enrollment"/>
    <rdfs:range rdf:resource="http://www.w3.org/2001/XMLSchema#string"/>
  </owl:DatatypeProperty>
  <owl:DatatypeProperty rdf:about="http://example.org/onto/prop/google_eventarc_enrollment_name">
    <rdfs:label>name</rdfs:label>
    <rdfs:comment>Resource name of the form
projects/{project}/locations/{location}/enrollments/{enrollment}</rdfs:comment>
    <rdfs:domain rdf:resource="http://example.org/onto/class/google_eventarc_enrollment"/>
    <rdfs:range rdf:resource="http://www.w3.org/2001/XMLSchema#string"/>
  </owl:DatatypeProperty>
  <owl:DatatypeProperty rdf:about="http://example.org/onto/prop/google_eventarc_enrollment_project">
    <rdfs:label>project</rdfs:label>
    <rdfs:domain rdf:resource="http://example.org/onto/class/google_eventarc_enrollment"/>
    <rdfs:range rdf:resource="http://www.w3.org/2001/XMLSchema#string"/>
  </owl:DatatypeProperty>
  <owl:DatatypeProperty rdf:about="http://example.org/onto/prop/google_eventarc_enrollment_terraform_labels">
    <rdfs:label>terraform_labels</rdfs:label>
    <rdfs:comment>The combination of labels configured directly on the resource
 and default labels configured on the provider.</rdfs:comment>
    <rdfs:domain rdf:resource="http://example.org/onto/class/google_eventarc_enrollment"/>
    <rdfs:range rdf:resource="http://www.w3.org/2001/XMLSchema#string"/>
  </owl:DatatypeProperty>
  <owl:DatatypeProperty rdf:about="http://example.org/onto/prop/google_eventarc_enrollment_uid">
    <rdfs:label>uid</rdfs:label>
    <rdfs:comment>Server assigned unique identifier for the channel. The value is a UUID4
string and guaranteed to remain unchanged until the resource is deleted.</rdfs:comment>
    <rdfs:domain rdf:resource="http://example.org/onto/class/google_eventarc_enrollment"/>
    <rdfs:range rdf:resource="http://www.w3.org/2001/XMLSchema#string"/>
  </owl:DatatypeProperty>
  <owl:DatatypeProperty rdf:about="http://example.org/onto/prop/google_eventarc_enrollment_update_time">
    <rdfs:label>update_time</rdfs:label>
    <rdfs:comment>The last-modified time.</rdfs:comment>
    <rdfs:domain rdf:resource="http://example.org/onto/class/google_eventarc_enrollment"/>
    <rdfs:range rdf:resource="http://www.w3.org/2001/XMLSchema#string"/>
  </owl:DatatypeProperty>
  <owl:DatatypeProperty rdf:about="http://example.org/onto/prop/google_eventarc_enrollment_create">
    <rdfs:label>create</rdfs:label>
    <rdfs:domain rdf:resource="http://example.org/onto/class/google_eventarc_enrollment"/>
    <rdfs:range rdf:resource="http://www.w3.org/2001/XMLSchema#string"/>
  </owl:DatatypeProperty>
  <owl:DatatypeProperty rdf:about="http://example.org/onto/prop/google_eventarc_enrollment_delete">
    <rdfs:label>delete</rdfs:label>
    <rdfs:domain rdf:resource="http://example.org/onto/class/google_eventarc_enrollment"/>
    <rdfs:range rdf:resource="http://www.w3.org/2001/XMLSchema#string"/>
  </owl:DatatypeProperty>
  <owl:DatatypeProperty rdf:about="http://example.org/onto/prop/google_eventarc_enrollment_update">
    <rdfs:label>update</rdfs:label>
    <rdfs:domain rdf:resource="http://example.org/onto/class/google_eventarc_enrollment"/>
    <rdfs:range rdf:resource="http://www.w3.org/2001/XMLSchema#string"/>
  </owl:DatatypeProperty>
</rdf:RDF>
