<?xml version="1.0" encoding="UTF-8"?>
<rdf:RDF
  xmlns:rdf="http://www.w3.org/1999/02/22-rdf-syntax-ns#"
  xmlns:rdfs="http://www.w3.org/2000/01/rdf-schema#"
  xmlns:owl="http://www.w3.org/2002/07/owl#"
  xmlns:xsd="http://www.w3.org/2001/XMLSchema#"
  xml:base="http://example.org/onto/">
  <owl:Class rdf:about="http://example.org/onto/class/google_recaptcha_enterprise_key">
    <rdfs:label>google_recaptcha_enterprise_key</rdfs:label>
    <rdfs:comment>#
#     ***     AUTO GENERATED CODE    ***    Type: DCL     ***
#
# ----------------------------------------------------------------------------
#
#     This file is managed by Magic Modules (https:#github.com/GoogleCloudPlatform/magic-modules)
#     and is based on the DCL (https:#github.com/GoogleCloudPlatform/declarative-resource-client-library).
#     Changes will need to be made to the DCL or Magic Modules instead of here.
#
#     We are not currently able to accept contributions to this file. If changes
#     are required, please file an issue at https:#github.com/hashicorp/terraform-provider-google/issues/new/choose
#
# ----------------------------------------------------------------------------
subcategory: "RecaptchaEnterprise"
description: |-
  The RecaptchaEnterprise Key resource
---</rdfs:comment>
  </owl:Class>
  <owl:DatatypeProperty rdf:about="http://example.org/onto/prop/google_recaptcha_enterprise_key_create_time">
    <rdfs:label>create_time</rdfs:label>
    <rdfs:comment>The timestamp corresponding to the creation of this Key.</rdfs:comment>
    <rdfs:domain rdf:resource="http://example.org/onto/class/google_recaptcha_enterprise_key"/>
    <rdfs:range rdf:resource="http://www.w3.org/2001/XMLSchema#string"/>
  </owl:DatatypeProperty>
  <owl:DatatypeProperty rdf:about="http://example.org/onto/prop/google_recaptcha_enterprise_key_display_name">
    <rdfs:label>display_name</rdfs:label>
    <rdfs:comment>Human-readable display name of this key. Modifiable by user.</rdfs:comment>
    <rdfs:domain rdf:resource="http://example.org/onto/class/google_recaptcha_enterprise_key"/>
    <rdfs:range rdf:resource="http://www.w3.org/2001/XMLSchema#string"/>
  </owl:DatatypeProperty>
  <owl:DatatypeProperty rdf:about="http://example.org/onto/prop/google_recaptcha_enterprise_key_effective_labels">
    <rdfs:label>effective_labels</rdfs:label>
    <rdfs:comment>All of labels (key/value pairs) present on the resource in GCP, including the labels configured through Terraform, other clients and services.</rdfs:comment>
    <rdfs:domain rdf:resource="http://example.org/onto/class/google_recaptcha_enterprise_key"/>
    <rdfs:range rdf:resource="http://www.w3.org/2001/XMLSchema#string"/>
  </owl:DatatypeProperty>
  <owl:DatatypeProperty rdf:about="http://example.org/onto/prop/google_recaptcha_enterprise_key_id">
    <rdfs:label>id</rdfs:label>
    <rdfs:domain rdf:resource="http://example.org/onto/class/google_recaptcha_enterprise_key"/>
    <rdfs:range rdf:resource="http://www.w3.org/2001/XMLSchema#string"/>
  </owl:DatatypeProperty>
  <owl:DatatypeProperty rdf:about="http://example.org/onto/prop/google_recaptcha_enterprise_key_labels">
    <rdfs:label>labels</rdfs:label>
    <rdfs:comment>See [Creating and managing labels](https://cloud.google.com/recaptcha-enterprise/docs/labels).

**Note**: This field is non-authoritative, and will only manage the labels present in your configuration.
Please refer to the field `effective_labels` for all of the labels present on the resource.</rdfs:comment>
    <rdfs:domain rdf:resource="http://example.org/onto/class/google_recaptcha_enterprise_key"/>
    <rdfs:range rdf:resource="http://www.w3.org/2001/XMLSchema#string"/>
  </owl:DatatypeProperty>
  <owl:DatatypeProperty rdf:about="http://example.org/onto/prop/google_recaptcha_enterprise_key_name">
    <rdfs:label>name</rdfs:label>
    <rdfs:comment>The resource id for the Key, which is the same as the Site Key itself.</rdfs:comment>
    <rdfs:domain rdf:resource="http://example.org/onto/class/google_recaptcha_enterprise_key"/>
    <rdfs:range rdf:resource="http://www.w3.org/2001/XMLSchema#string"/>
  </owl:DatatypeProperty>
  <owl:DatatypeProperty rdf:about="http://example.org/onto/prop/google_recaptcha_enterprise_key_project">
    <rdfs:label>project</rdfs:label>
    <rdfs:comment>The project for the resource</rdfs:comment>
    <rdfs:domain rdf:resource="http://example.org/onto/class/google_recaptcha_enterprise_key"/>
    <rdfs:range rdf:resource="http://www.w3.org/2001/XMLSchema#string"/>
  </owl:DatatypeProperty>
  <owl:DatatypeProperty rdf:about="http://example.org/onto/prop/google_recaptcha_enterprise_key_terraform_labels">
    <rdfs:label>terraform_labels</rdfs:label>
    <rdfs:comment>The combination of labels configured directly on the resource and default labels configured on the provider.</rdfs:comment>
    <rdfs:domain rdf:resource="http://example.org/onto/class/google_recaptcha_enterprise_key"/>
    <rdfs:range rdf:resource="http://www.w3.org/2001/XMLSchema#string"/>
  </owl:DatatypeProperty>
  <owl:DatatypeProperty rdf:about="http://example.org/onto/prop/google_recaptcha_enterprise_key_allow_all_package_names">
    <rdfs:label>allow_all_package_names</rdfs:label>
    <rdfs:comment>If set to true, it means allowed_package_names will not be enforced.</rdfs:comment>
    <rdfs:domain rdf:resource="http://example.org/onto/class/google_recaptcha_enterprise_key"/>
    <rdfs:range rdf:resource="http://www.w3.org/2001/XMLSchema#string"/>
  </owl:DatatypeProperty>
  <owl:DatatypeProperty rdf:about="http://example.org/onto/prop/google_recaptcha_enterprise_key_allowed_package_names">
    <rdfs:label>allowed_package_names</rdfs:label>
    <rdfs:comment>Android package names of apps allowed to use the key. Example: 'com.companyname.appname'</rdfs:comment>
    <rdfs:domain rdf:resource="http://example.org/onto/class/google_recaptcha_enterprise_key"/>
    <rdfs:range rdf:resource="http://www.w3.org/2001/XMLSchema#string"/>
  </owl:DatatypeProperty>
  <owl:DatatypeProperty rdf:about="http://example.org/onto/prop/google_recaptcha_enterprise_key_allow_all_bundle_ids">
    <rdfs:label>allow_all_bundle_ids</rdfs:label>
    <rdfs:comment>If set to true, it means allowed_bundle_ids will not be enforced.</rdfs:comment>
    <rdfs:domain rdf:resource="http://example.org/onto/class/google_recaptcha_enterprise_key"/>
    <rdfs:range rdf:resource="http://www.w3.org/2001/XMLSchema#string"/>
  </owl:DatatypeProperty>
  <owl:DatatypeProperty rdf:about="http://example.org/onto/prop/google_recaptcha_enterprise_key_allowed_bundle_ids">
    <rdfs:label>allowed_bundle_ids</rdfs:label>
    <rdfs:comment>iOS bundle ids of apps allowed to use the key. Example: 'com.companyname.productname.appname'</rdfs:comment>
    <rdfs:domain rdf:resource="http://example.org/onto/class/google_recaptcha_enterprise_key"/>
    <rdfs:range rdf:resource="http://www.w3.org/2001/XMLSchema#string"/>
  </owl:DatatypeProperty>
  <owl:DatatypeProperty rdf:about="http://example.org/onto/prop/google_recaptcha_enterprise_key_testing_challenge">
    <rdfs:label>testing_challenge</rdfs:label>
    <rdfs:comment>For challenge-based keys only (CHECKBOX, INVISIBLE), all challenge requests for this site will return nocaptcha if NOCAPTCHA, or an unsolvable challenge if UNSOLVABLE_CHALLENGE. Possible values: TESTING_CHALLENGE_UNSPECIFIED, NOCAPTCHA, UNSOLVABLE_CHALLENGE</rdfs:comment>
    <rdfs:domain rdf:resource="http://example.org/onto/class/google_recaptcha_enterprise_key"/>
    <rdfs:range rdf:resource="http://www.w3.org/2001/XMLSchema#string"/>
  </owl:DatatypeProperty>
  <owl:DatatypeProperty rdf:about="http://example.org/onto/prop/google_recaptcha_enterprise_key_testing_score">
    <rdfs:label>testing_score</rdfs:label>
    <rdfs:comment>All assessments for this Key will return this score. Must be between 0 (likely not legitimate) and 1 (likely legitimate) inclusive.</rdfs:comment>
    <rdfs:domain rdf:resource="http://example.org/onto/class/google_recaptcha_enterprise_key"/>
    <rdfs:range rdf:resource="http://www.w3.org/2001/XMLSchema#string"/>
  </owl:DatatypeProperty>
  <owl:DatatypeProperty rdf:about="http://example.org/onto/prop/google_recaptcha_enterprise_key_create">
    <rdfs:label>create</rdfs:label>
    <rdfs:domain rdf:resource="http://example.org/onto/class/google_recaptcha_enterprise_key"/>
    <rdfs:range rdf:resource="http://www.w3.org/2001/XMLSchema#string"/>
  </owl:DatatypeProperty>
  <owl:DatatypeProperty rdf:about="http://example.org/onto/prop/google_recaptcha_enterprise_key_delete">
    <rdfs:label>delete</rdfs:label>
    <rdfs:domain rdf:resource="http://example.org/onto/class/google_recaptcha_enterprise_key"/>
    <rdfs:range rdf:resource="http://www.w3.org/2001/XMLSchema#string"/>
  </owl:DatatypeProperty>
  <owl:DatatypeProperty rdf:about="http://example.org/onto/prop/google_recaptcha_enterprise_key_update">
    <rdfs:label>update</rdfs:label>
    <rdfs:domain rdf:resource="http://example.org/onto/class/google_recaptcha_enterprise_key"/>
    <rdfs:range rdf:resource="http://www.w3.org/2001/XMLSchema#string"/>
  </owl:DatatypeProperty>
  <owl:DatatypeProperty rdf:about="http://example.org/onto/prop/google_recaptcha_enterprise_key_waf_feature">
    <rdfs:label>waf_feature</rdfs:label>
    <rdfs:comment>Supported WAF features. For more information, see https://cloud.google.com/recaptcha-enterprise/docs/usecase#comparison_of_features. Possible values: CHALLENGE_PAGE, SESSION_TOKEN, ACTION_TOKEN, EXPRESS</rdfs:comment>
    <rdfs:domain rdf:resource="http://example.org/onto/class/google_recaptcha_enterprise_key"/>
    <rdfs:range rdf:resource="http://www.w3.org/2001/XMLSchema#string"/>
  </owl:DatatypeProperty>
  <owl:DatatypeProperty rdf:about="http://example.org/onto/prop/google_recaptcha_enterprise_key_waf_service">
    <rdfs:label>waf_service</rdfs:label>
    <rdfs:comment>The WAF service that uses this key. Possible values: CA, FASTLY</rdfs:comment>
    <rdfs:domain rdf:resource="http://example.org/onto/class/google_recaptcha_enterprise_key"/>
    <rdfs:range rdf:resource="http://www.w3.org/2001/XMLSchema#string"/>
  </owl:DatatypeProperty>
  <owl:DatatypeProperty rdf:about="http://example.org/onto/prop/google_recaptcha_enterprise_key_allow_all_domains">
    <rdfs:label>allow_all_domains</rdfs:label>
    <rdfs:comment>If set to true, it means allowed_domains will not be enforced.</rdfs:comment>
    <rdfs:domain rdf:resource="http://example.org/onto/class/google_recaptcha_enterprise_key"/>
    <rdfs:range rdf:resource="http://www.w3.org/2001/XMLSchema#string"/>
  </owl:DatatypeProperty>
  <owl:DatatypeProperty rdf:about="http://example.org/onto/prop/google_recaptcha_enterprise_key_allow_amp_traffic">
    <rdfs:label>allow_amp_traffic</rdfs:label>
    <rdfs:comment>If set to true, the key can be used on AMP (Accelerated Mobile Pages) websites. This is supported only for the SCORE integration type.</rdfs:comment>
    <rdfs:domain rdf:resource="http://example.org/onto/class/google_recaptcha_enterprise_key"/>
    <rdfs:range rdf:resource="http://www.w3.org/2001/XMLSchema#string"/>
  </owl:DatatypeProperty>
  <owl:DatatypeProperty rdf:about="http://example.org/onto/prop/google_recaptcha_enterprise_key_allowed_domains">
    <rdfs:label>allowed_domains</rdfs:label>
    <rdfs:comment>Domains or subdomains of websites allowed to use the key. All subdomains of an allowed domain are automatically allowed. A valid domain requires a host and must not include any path, port, query or fragment. Examples: 'example.com' or 'subdomain.example.com'</rdfs:comment>
    <rdfs:domain rdf:resource="http://example.org/onto/class/google_recaptcha_enterprise_key"/>
    <rdfs:range rdf:resource="http://www.w3.org/2001/XMLSchema#string"/>
  </owl:DatatypeProperty>
  <owl:DatatypeProperty rdf:about="http://example.org/onto/prop/google_recaptcha_enterprise_key_challenge_security_preference">
    <rdfs:label>challenge_security_preference</rdfs:label>
    <rdfs:comment>Settings for the frequency and difficulty at which this key triggers captcha challenges. This should only be specified for IntegrationTypes CHECKBOX and INVISIBLE. Possible values: CHALLENGE_SECURITY_PREFERENCE_UNSPECIFIED, USABILITY, BALANCE, SECURITY</rdfs:comment>
    <rdfs:domain rdf:resource="http://example.org/onto/class/google_recaptcha_enterprise_key"/>
    <rdfs:range rdf:resource="http://www.w3.org/2001/XMLSchema#string"/>
  </owl:DatatypeProperty>
  <owl:DatatypeProperty rdf:about="http://example.org/onto/prop/google_recaptcha_enterprise_key_integration_type">
    <rdfs:label>integration_type</rdfs:label>
    <rdfs:comment>Required. Describes how this key is integrated with the website. Possible values: SCORE, CHECKBOX, INVISIBLE</rdfs:comment>
    <rdfs:domain rdf:resource="http://example.org/onto/class/google_recaptcha_enterprise_key"/>
    <rdfs:range rdf:resource="http://www.w3.org/2001/XMLSchema#string"/>
  </owl:DatatypeProperty>
</rdf:RDF>
