<?xml version="1.0" encoding="UTF-8"?>
<rdf:RDF
  xmlns:rdf="http://www.w3.org/1999/02/22-rdf-syntax-ns#"
  xmlns:rdfs="http://www.w3.org/2000/01/rdf-schema#"
  xmlns:owl="http://www.w3.org/2002/07/owl#"
  xmlns:xsd="http://www.w3.org/2001/XMLSchema#"
  xml:base="http://example.org/onto/">
  <owl:Class rdf:about="http://example.org/onto/class/google_vertex_ai_featurestore">
    <rdfs:label>google_vertex_ai_featurestore</rdfs:label>
    <rdfs:comment>#
#     ***     AUTO GENERATED CODE    ***    Type: MMv1     ***
#
# ----------------------------------------------------------------------------
#
#     This code is generated by Magic Modules using the following:
#
#     Configuration: https:#github.com/GoogleCloudPlatform/magic-modules/tree/main/mmv1/products/vertexai/Featurestore.yaml
#     Template:      https:#github.com/GoogleCloudPlatform/magic-modules/tree/main/mmv1/templates/terraform/resource.html.markdown.tmpl
#
#     DO NOT EDIT this file directly. Any changes made to this file will be
#     overwritten during the next generation cycle.
#
# ----------------------------------------------------------------------------
subcategory: "Vertex AI"
description: |-
  A collection of DataItems and Annotations on them.
---</rdfs:comment>
  </owl:Class>
  <owl:DatatypeProperty rdf:about="http://example.org/onto/prop/google_vertex_ai_featurestore_create_time">
    <rdfs:label>create_time</rdfs:label>
    <rdfs:comment>The timestamp of when the featurestore was created in RFC3339 UTC "Zulu" format, with nanosecond resolution and up to nine fractional digits.</rdfs:comment>
    <rdfs:domain rdf:resource="http://example.org/onto/class/google_vertex_ai_featurestore"/>
    <rdfs:range rdf:resource="http://www.w3.org/2001/XMLSchema#string"/>
  </owl:DatatypeProperty>
  <owl:DatatypeProperty rdf:about="http://example.org/onto/prop/google_vertex_ai_featurestore_effective_labels">
    <rdfs:label>effective_labels</rdfs:label>
    <rdfs:comment>All of labels (key/value pairs) present on the resource in GCP, including the labels configured through Terraform, other clients and services.</rdfs:comment>
    <rdfs:domain rdf:resource="http://example.org/onto/class/google_vertex_ai_featurestore"/>
    <rdfs:range rdf:resource="http://www.w3.org/2001/XMLSchema#string"/>
  </owl:DatatypeProperty>
  <owl:DatatypeProperty rdf:about="http://example.org/onto/prop/google_vertex_ai_featurestore_etag">
    <rdfs:label>etag</rdfs:label>
    <rdfs:comment>Used to perform consistent read-modify-write updates.</rdfs:comment>
    <rdfs:domain rdf:resource="http://example.org/onto/class/google_vertex_ai_featurestore"/>
    <rdfs:range rdf:resource="http://www.w3.org/2001/XMLSchema#string"/>
  </owl:DatatypeProperty>
  <owl:DatatypeProperty rdf:about="http://example.org/onto/prop/google_vertex_ai_featurestore_force_destroy">
    <rdfs:label>force_destroy</rdfs:label>
    <rdfs:comment>If set to true, any EntityTypes and Features for this Featurestore will also be deleted</rdfs:comment>
    <rdfs:domain rdf:resource="http://example.org/onto/class/google_vertex_ai_featurestore"/>
    <rdfs:range rdf:resource="http://www.w3.org/2001/XMLSchema#string"/>
  </owl:DatatypeProperty>
  <owl:DatatypeProperty rdf:about="http://example.org/onto/prop/google_vertex_ai_featurestore_id">
    <rdfs:label>id</rdfs:label>
    <rdfs:domain rdf:resource="http://example.org/onto/class/google_vertex_ai_featurestore"/>
    <rdfs:range rdf:resource="http://www.w3.org/2001/XMLSchema#string"/>
  </owl:DatatypeProperty>
  <owl:DatatypeProperty rdf:about="http://example.org/onto/prop/google_vertex_ai_featurestore_labels">
    <rdfs:label>labels</rdfs:label>
    <rdfs:comment>A set of key/value label pairs to assign to this Featurestore.


**Note**: This field is non-authoritative, and will only manage the labels present in your configuration.
Please refer to the field 'effective_labels' for all of the labels present on the resource.</rdfs:comment>
    <rdfs:domain rdf:resource="http://example.org/onto/class/google_vertex_ai_featurestore"/>
    <rdfs:range rdf:resource="http://www.w3.org/2001/XMLSchema#string"/>
  </owl:DatatypeProperty>
  <owl:DatatypeProperty rdf:about="http://example.org/onto/prop/google_vertex_ai_featurestore_name">
    <rdfs:label>name</rdfs:label>
    <rdfs:comment>The name of the Featurestore. This value may be up to 60 characters, and valid characters are [a-z0-9_]. The first character cannot be a number.</rdfs:comment>
    <rdfs:domain rdf:resource="http://example.org/onto/class/google_vertex_ai_featurestore"/>
    <rdfs:range rdf:resource="http://www.w3.org/2001/XMLSchema#string"/>
  </owl:DatatypeProperty>
  <owl:DatatypeProperty rdf:about="http://example.org/onto/prop/google_vertex_ai_featurestore_project">
    <rdfs:label>project</rdfs:label>
    <rdfs:domain rdf:resource="http://example.org/onto/class/google_vertex_ai_featurestore"/>
    <rdfs:range rdf:resource="http://www.w3.org/2001/XMLSchema#string"/>
  </owl:DatatypeProperty>
  <owl:DatatypeProperty rdf:about="http://example.org/onto/prop/google_vertex_ai_featurestore_region">
    <rdfs:label>region</rdfs:label>
    <rdfs:comment>The region of the dataset. eg us-central1</rdfs:comment>
    <rdfs:domain rdf:resource="http://example.org/onto/class/google_vertex_ai_featurestore"/>
    <rdfs:range rdf:resource="http://www.w3.org/2001/XMLSchema#string"/>
  </owl:DatatypeProperty>
  <owl:DatatypeProperty rdf:about="http://example.org/onto/prop/google_vertex_ai_featurestore_terraform_labels">
    <rdfs:label>terraform_labels</rdfs:label>
    <rdfs:comment>The combination of labels configured directly on the resource
 and default labels configured on the provider.</rdfs:comment>
    <rdfs:domain rdf:resource="http://example.org/onto/class/google_vertex_ai_featurestore"/>
    <rdfs:range rdf:resource="http://www.w3.org/2001/XMLSchema#string"/>
  </owl:DatatypeProperty>
  <owl:DatatypeProperty rdf:about="http://example.org/onto/prop/google_vertex_ai_featurestore_update_time">
    <rdfs:label>update_time</rdfs:label>
    <rdfs:comment>The timestamp of when the featurestore was last updated in RFC3339 UTC "Zulu" format, with nanosecond resolution and up to nine fractional digits.</rdfs:comment>
    <rdfs:domain rdf:resource="http://example.org/onto/class/google_vertex_ai_featurestore"/>
    <rdfs:range rdf:resource="http://www.w3.org/2001/XMLSchema#string"/>
  </owl:DatatypeProperty>
  <owl:DatatypeProperty rdf:about="http://example.org/onto/prop/google_vertex_ai_featurestore_kms_key_name">
    <rdfs:label>kms_key_name</rdfs:label>
    <rdfs:comment>The Cloud KMS resource identifier of the customer managed encryption key used to protect a resource. Has the form: projects/my-project/locations/my-region/keyRings/my-kr/cryptoKeys/my-key. The key needs to be in the same region as where the compute resource is created.</rdfs:comment>
    <rdfs:domain rdf:resource="http://example.org/onto/class/google_vertex_ai_featurestore"/>
    <rdfs:range rdf:resource="http://www.w3.org/2001/XMLSchema#string"/>
  </owl:DatatypeProperty>
  <owl:DatatypeProperty rdf:about="http://example.org/onto/prop/google_vertex_ai_featurestore_fixed_node_count">
    <rdfs:label>fixed_node_count</rdfs:label>
    <rdfs:comment>The number of nodes for each cluster. The number of nodes will not scale automatically but can be scaled manually by providing different values when updating.</rdfs:comment>
    <rdfs:domain rdf:resource="http://example.org/onto/class/google_vertex_ai_featurestore"/>
    <rdfs:range rdf:resource="http://www.w3.org/2001/XMLSchema#string"/>
  </owl:DatatypeProperty>
  <owl:DatatypeProperty rdf:about="http://example.org/onto/prop/google_vertex_ai_featurestore_max_node_count">
    <rdfs:label>max_node_count</rdfs:label>
    <rdfs:comment>The maximum number of nodes to scale up to. Must be greater than minNodeCount, and less than or equal to 10 times of 'minNodeCount'.</rdfs:comment>
    <rdfs:domain rdf:resource="http://example.org/onto/class/google_vertex_ai_featurestore"/>
    <rdfs:range rdf:resource="http://www.w3.org/2001/XMLSchema#string"/>
  </owl:DatatypeProperty>
  <owl:DatatypeProperty rdf:about="http://example.org/onto/prop/google_vertex_ai_featurestore_min_node_count">
    <rdfs:label>min_node_count</rdfs:label>
    <rdfs:comment>The minimum number of nodes to scale down to. Must be greater than or equal to 1.</rdfs:comment>
    <rdfs:domain rdf:resource="http://example.org/onto/class/google_vertex_ai_featurestore"/>
    <rdfs:range rdf:resource="http://www.w3.org/2001/XMLSchema#string"/>
  </owl:DatatypeProperty>
  <owl:DatatypeProperty rdf:about="http://example.org/onto/prop/google_vertex_ai_featurestore_create">
    <rdfs:label>create</rdfs:label>
    <rdfs:domain rdf:resource="http://example.org/onto/class/google_vertex_ai_featurestore"/>
    <rdfs:range rdf:resource="http://www.w3.org/2001/XMLSchema#string"/>
  </owl:DatatypeProperty>
  <owl:DatatypeProperty rdf:about="http://example.org/onto/prop/google_vertex_ai_featurestore_delete">
    <rdfs:label>delete</rdfs:label>
    <rdfs:domain rdf:resource="http://example.org/onto/class/google_vertex_ai_featurestore"/>
    <rdfs:range rdf:resource="http://www.w3.org/2001/XMLSchema#string"/>
  </owl:DatatypeProperty>
  <owl:DatatypeProperty rdf:about="http://example.org/onto/prop/google_vertex_ai_featurestore_update">
    <rdfs:label>update</rdfs:label>
    <rdfs:domain rdf:resource="http://example.org/onto/class/google_vertex_ai_featurestore"/>
    <rdfs:range rdf:resource="http://www.w3.org/2001/XMLSchema#string"/>
  </owl:DatatypeProperty>
</rdf:RDF>
