<?xml version="1.0" encoding="UTF-8"?>
<rdf:RDF
  xmlns:rdf="http://www.w3.org/1999/02/22-rdf-syntax-ns#"
  xmlns:rdfs="http://www.w3.org/2000/01/rdf-schema#"
  xmlns:owl="http://www.w3.org/2002/07/owl#"
  xmlns:xsd="http://www.w3.org/2001/XMLSchema#"
  xml:base="http://example.org/onto/">
  <owl:Class rdf:about="http://example.org/onto/class/google_bigquery_datapolicyv2_data_policy">
    <rdfs:label>google_bigquery_datapolicyv2_data_policy</rdfs:label>
    <rdfs:comment>#
#     ***     AUTO GENERATED CODE    ***    Type: MMv1     ***
#
# ----------------------------------------------------------------------------
#
#     This code is generated by Magic Modules using the following:
#
#     Configuration: https:#github.com/GoogleCloudPlatform/magic-modules/tree/main/mmv1/products/bigquerydatapolicyv2/DataPolicy.yaml
#     Template:      https:#github.com/GoogleCloudPlatform/magic-modules/tree/main/mmv1/templates/terraform/resource.html.markdown.tmpl
#
#     DO NOT EDIT this file directly. Any changes made to this file will be
#     overwritten during the next generation cycle.
#
# ----------------------------------------------------------------------------
subcategory: "BigQuery Data Policy V2"
description: |-
  BigQuery Data Policy
---</rdfs:comment>
  </owl:Class>
  <owl:DatatypeProperty rdf:about="http://example.org/onto/prop/google_bigquery_datapolicyv2_data_policy_data_policy_id">
    <rdfs:label>data_policy_id</rdfs:label>
    <rdfs:comment>User-assigned (human readable) ID of the data policy that needs to be
unique within a project. Used as {data_policy_id} in part of the resource
name.</rdfs:comment>
    <rdfs:domain rdf:resource="http://example.org/onto/class/google_bigquery_datapolicyv2_data_policy"/>
    <rdfs:range rdf:resource="http://www.w3.org/2001/XMLSchema#string"/>
  </owl:DatatypeProperty>
  <owl:DatatypeProperty rdf:about="http://example.org/onto/prop/google_bigquery_datapolicyv2_data_policy_data_policy_type">
    <rdfs:label>data_policy_type</rdfs:label>
    <rdfs:comment>Type of data policy.
Possible values:
DATA_MASKING_POLICY
RAW_DATA_ACCESS_POLICY
COLUMN_LEVEL_SECURITY_POLICY</rdfs:comment>
    <rdfs:domain rdf:resource="http://example.org/onto/class/google_bigquery_datapolicyv2_data_policy"/>
    <rdfs:range rdf:resource="http://www.w3.org/2001/XMLSchema#string"/>
  </owl:DatatypeProperty>
  <owl:DatatypeProperty rdf:about="http://example.org/onto/prop/google_bigquery_datapolicyv2_data_policy_etag">
    <rdfs:label>etag</rdfs:label>
    <rdfs:comment>The etag for this Data Policy.
This field is used for UpdateDataPolicy calls. If Data Policy exists, this
field is required and must match the server's etag. It will also be
populated in the response of GetDataPolicy, CreateDataPolicy, and
UpdateDataPolicy calls.</rdfs:comment>
    <rdfs:domain rdf:resource="http://example.org/onto/class/google_bigquery_datapolicyv2_data_policy"/>
    <rdfs:range rdf:resource="http://www.w3.org/2001/XMLSchema#string"/>
  </owl:DatatypeProperty>
  <owl:DatatypeProperty rdf:about="http://example.org/onto/prop/google_bigquery_datapolicyv2_data_policy_grantees">
    <rdfs:label>grantees</rdfs:label>
    <rdfs:comment>The list of IAM principals that have Fine Grained Access to the underlying
data goverened by this data policy.

Uses the [IAM V2 principal
syntax](https://cloud.google.com/iam/docs/principal-identifiers#v2) Only
supports principal types users, groups, serviceaccounts, cloudidentity.
This field is supported in V2 Data Policy only. In case of V1 data policies
(i.e. verion = 1 and policy_tag is set), this field is not populated.</rdfs:comment>
    <rdfs:domain rdf:resource="http://example.org/onto/class/google_bigquery_datapolicyv2_data_policy"/>
    <rdfs:range rdf:resource="http://www.w3.org/2001/XMLSchema#string"/>
  </owl:DatatypeProperty>
  <owl:DatatypeProperty rdf:about="http://example.org/onto/prop/google_bigquery_datapolicyv2_data_policy_id">
    <rdfs:label>id</rdfs:label>
    <rdfs:domain rdf:resource="http://example.org/onto/class/google_bigquery_datapolicyv2_data_policy"/>
    <rdfs:range rdf:resource="http://www.w3.org/2001/XMLSchema#string"/>
  </owl:DatatypeProperty>
  <owl:DatatypeProperty rdf:about="http://example.org/onto/prop/google_bigquery_datapolicyv2_data_policy_location">
    <rdfs:label>location</rdfs:label>
    <rdfs:comment>Resource ID segment making up resource 'name'. It identifies the resource within its parent collection as described in https://google.aip.dev/122.</rdfs:comment>
    <rdfs:domain rdf:resource="http://example.org/onto/class/google_bigquery_datapolicyv2_data_policy"/>
    <rdfs:range rdf:resource="http://www.w3.org/2001/XMLSchema#string"/>
  </owl:DatatypeProperty>
  <owl:DatatypeProperty rdf:about="http://example.org/onto/prop/google_bigquery_datapolicyv2_data_policy_name">
    <rdfs:label>name</rdfs:label>
    <rdfs:comment>Identifier. Resource name of this data policy, in the format of
'projects/{project_number}/locations/{location_id}/dataPolicies/{data_policy_id}'.</rdfs:comment>
    <rdfs:domain rdf:resource="http://example.org/onto/class/google_bigquery_datapolicyv2_data_policy"/>
    <rdfs:range rdf:resource="http://www.w3.org/2001/XMLSchema#string"/>
  </owl:DatatypeProperty>
  <owl:DatatypeProperty rdf:about="http://example.org/onto/prop/google_bigquery_datapolicyv2_data_policy_policy_tag">
    <rdfs:label>policy_tag</rdfs:label>
    <rdfs:comment>Policy tag resource name, in the format of
'projects/{project_number}/locations/{location_id}/taxonomies/{taxonomy_id}/policyTags/{policyTag_id}'.
policy_tag is supported only for V1 data policies.</rdfs:comment>
    <rdfs:domain rdf:resource="http://example.org/onto/class/google_bigquery_datapolicyv2_data_policy"/>
    <rdfs:range rdf:resource="http://www.w3.org/2001/XMLSchema#string"/>
  </owl:DatatypeProperty>
  <owl:DatatypeProperty rdf:about="http://example.org/onto/prop/google_bigquery_datapolicyv2_data_policy_project">
    <rdfs:label>project</rdfs:label>
    <rdfs:domain rdf:resource="http://example.org/onto/class/google_bigquery_datapolicyv2_data_policy"/>
    <rdfs:range rdf:resource="http://www.w3.org/2001/XMLSchema#string"/>
  </owl:DatatypeProperty>
  <owl:DatatypeProperty rdf:about="http://example.org/onto/prop/google_bigquery_datapolicyv2_data_policy_version">
    <rdfs:label>version</rdfs:label>
    <rdfs:comment>The version of the Data Policy resource.
Possible values:
V1
V2</rdfs:comment>
    <rdfs:domain rdf:resource="http://example.org/onto/class/google_bigquery_datapolicyv2_data_policy"/>
    <rdfs:range rdf:resource="http://www.w3.org/2001/XMLSchema#string"/>
  </owl:DatatypeProperty>
  <owl:DatatypeProperty rdf:about="http://example.org/onto/prop/google_bigquery_datapolicyv2_data_policy_predefined_expression">
    <rdfs:label>predefined_expression</rdfs:label>
    <rdfs:comment>A predefined masking expression.
Possible values:
SHA256
ALWAYS_NULL
DEFAULT_MASKING_VALUE
LAST_FOUR_CHARACTERS
FIRST_FOUR_CHARACTERS
EMAIL_MASK
DATE_YEAR_MASK
RANDOM_HASH</rdfs:comment>
    <rdfs:domain rdf:resource="http://example.org/onto/class/google_bigquery_datapolicyv2_data_policy"/>
    <rdfs:range rdf:resource="http://www.w3.org/2001/XMLSchema#string"/>
  </owl:DatatypeProperty>
  <owl:DatatypeProperty rdf:about="http://example.org/onto/prop/google_bigquery_datapolicyv2_data_policy_routine">
    <rdfs:label>routine</rdfs:label>
    <rdfs:comment>The name of the BigQuery routine that contains the custom masking
routine, in the format of
'projects/{project_number}/datasets/{dataset_id}/routines/{routine_id}'.</rdfs:comment>
    <rdfs:domain rdf:resource="http://example.org/onto/class/google_bigquery_datapolicyv2_data_policy"/>
    <rdfs:range rdf:resource="http://www.w3.org/2001/XMLSchema#string"/>
  </owl:DatatypeProperty>
  <owl:DatatypeProperty rdf:about="http://example.org/onto/prop/google_bigquery_datapolicyv2_data_policy_create">
    <rdfs:label>create</rdfs:label>
    <rdfs:domain rdf:resource="http://example.org/onto/class/google_bigquery_datapolicyv2_data_policy"/>
    <rdfs:range rdf:resource="http://www.w3.org/2001/XMLSchema#string"/>
  </owl:DatatypeProperty>
  <owl:DatatypeProperty rdf:about="http://example.org/onto/prop/google_bigquery_datapolicyv2_data_policy_delete">
    <rdfs:label>delete</rdfs:label>
    <rdfs:domain rdf:resource="http://example.org/onto/class/google_bigquery_datapolicyv2_data_policy"/>
    <rdfs:range rdf:resource="http://www.w3.org/2001/XMLSchema#string"/>
  </owl:DatatypeProperty>
  <owl:DatatypeProperty rdf:about="http://example.org/onto/prop/google_bigquery_datapolicyv2_data_policy_update">
    <rdfs:label>update</rdfs:label>
    <rdfs:domain rdf:resource="http://example.org/onto/class/google_bigquery_datapolicyv2_data_policy"/>
    <rdfs:range rdf:resource="http://www.w3.org/2001/XMLSchema#string"/>
  </owl:DatatypeProperty>
</rdf:RDF>
