<?xml version="1.0" encoding="UTF-8"?>
<rdf:RDF
  xmlns:rdf="http://www.w3.org/1999/02/22-rdf-syntax-ns#"
  xmlns:rdfs="http://www.w3.org/2000/01/rdf-schema#"
  xmlns:owl="http://www.w3.org/2002/07/owl#"
  xmlns:xsd="http://www.w3.org/2001/XMLSchema#"
  xml:base="http://example.org/onto/">
  <owl:Class rdf:about="http://example.org/onto/class/google_chronicle_rule">
    <rdfs:label>google_chronicle_rule</rdfs:label>
    <rdfs:comment>#
#     ***     AUTO GENERATED CODE    ***    Type: MMv1     ***
#
# ----------------------------------------------------------------------------
#
#     This code is generated by Magic Modules using the following:
#
#     Configuration: https:#github.com/GoogleCloudPlatform/magic-modules/tree/main/mmv1/products/chronicle/Rule.yaml
#     Template:      https:#github.com/GoogleCloudPlatform/magic-modules/tree/main/mmv1/templates/terraform/resource.html.markdown.tmpl
#
#     DO NOT EDIT this file directly. Any changes made to this file will be
#     overwritten during the next generation cycle.
#
# ----------------------------------------------------------------------------
subcategory: "Chronicle"
description: |-
  The Rule resource represents a user-created rule.
---</rdfs:comment>
  </owl:Class>
  <owl:DatatypeProperty rdf:about="http://example.org/onto/prop/google_chronicle_rule_allowed_run_frequencies">
    <rdfs:label>allowed_run_frequencies</rdfs:label>
    <rdfs:comment>Output only. The run frequencies that are allowed for the rule.
Populated in BASIC view and FULL view.</rdfs:comment>
    <rdfs:domain rdf:resource="http://example.org/onto/class/google_chronicle_rule"/>
    <rdfs:range rdf:resource="http://www.w3.org/2001/XMLSchema#string"/>
  </owl:DatatypeProperty>
  <owl:DatatypeProperty rdf:about="http://example.org/onto/prop/google_chronicle_rule_author">
    <rdfs:label>author</rdfs:label>
    <rdfs:comment>Output only. The author of the rule. Extracted from the meta section of text.
Populated in BASIC view and FULL view.</rdfs:comment>
    <rdfs:domain rdf:resource="http://example.org/onto/class/google_chronicle_rule"/>
    <rdfs:range rdf:resource="http://www.w3.org/2001/XMLSchema#string"/>
  </owl:DatatypeProperty>
  <owl:DatatypeProperty rdf:about="http://example.org/onto/prop/google_chronicle_rule_compilation_diagnostics">
    <rdfs:label>compilation_diagnostics</rdfs:label>
    <rdfs:comment>Output only. A list of a rule's corresponding compilation diagnostic messages
such as compilation errors and compilation warnings.
Populated in FULL view.</rdfs:comment>
    <rdfs:domain rdf:resource="http://example.org/onto/class/google_chronicle_rule"/>
    <rdfs:range rdf:resource="http://www.w3.org/2001/XMLSchema#string"/>
  </owl:DatatypeProperty>
  <owl:DatatypeProperty rdf:about="http://example.org/onto/prop/google_chronicle_rule_compilation_state">
    <rdfs:label>compilation_state</rdfs:label>
    <rdfs:comment>Output only. The current compilation state of the rule.
Populated in FULL view.
Possible values:
COMPILATION_STATE_UNSPECIFIED
SUCCEEDED
FAILED</rdfs:comment>
    <rdfs:domain rdf:resource="http://example.org/onto/class/google_chronicle_rule"/>
    <rdfs:range rdf:resource="http://www.w3.org/2001/XMLSchema#string"/>
  </owl:DatatypeProperty>
  <owl:DatatypeProperty rdf:about="http://example.org/onto/prop/google_chronicle_rule_create_time">
    <rdfs:label>create_time</rdfs:label>
    <rdfs:comment>Output only. The timestamp of when the rule was created.
Populated in FULL view.</rdfs:comment>
    <rdfs:domain rdf:resource="http://example.org/onto/class/google_chronicle_rule"/>
    <rdfs:range rdf:resource="http://www.w3.org/2001/XMLSchema#string"/>
  </owl:DatatypeProperty>
  <owl:DatatypeProperty rdf:about="http://example.org/onto/prop/google_chronicle_rule_data_tables">
    <rdfs:label>data_tables</rdfs:label>
    <rdfs:comment>Output only. Resource names of the data tables used in this rule.</rdfs:comment>
    <rdfs:domain rdf:resource="http://example.org/onto/class/google_chronicle_rule"/>
    <rdfs:range rdf:resource="http://www.w3.org/2001/XMLSchema#string"/>
  </owl:DatatypeProperty>
  <owl:DatatypeProperty rdf:about="http://example.org/onto/prop/google_chronicle_rule_deletion_policy">
    <rdfs:label>deletion_policy</rdfs:label>
    <rdfs:comment>Policy to determine if the rule should be deleted forcefully.
If deletion_policy = "FORCE", any retrohunts and any detections associated with the rule
will also be deleted. If deletion_policy = "DEFAULT", the call will only succeed if the
rule has no associated retrohunts, including completed retrohunts, and no
associated detections. Regardless of this field's value, the rule
deployment associated with this rule will also be deleted.
Possible values: DEFAULT, FORCE</rdfs:comment>
    <rdfs:domain rdf:resource="http://example.org/onto/class/google_chronicle_rule"/>
    <rdfs:range rdf:resource="http://www.w3.org/2001/XMLSchema#string"/>
  </owl:DatatypeProperty>
  <owl:DatatypeProperty rdf:about="http://example.org/onto/prop/google_chronicle_rule_display_name">
    <rdfs:label>display_name</rdfs:label>
    <rdfs:comment>Output only. Display name of the rule.
Populated in BASIC view and FULL view.</rdfs:comment>
    <rdfs:domain rdf:resource="http://example.org/onto/class/google_chronicle_rule"/>
    <rdfs:range rdf:resource="http://www.w3.org/2001/XMLSchema#string"/>
  </owl:DatatypeProperty>
  <owl:DatatypeProperty rdf:about="http://example.org/onto/prop/google_chronicle_rule_etag">
    <rdfs:label>etag</rdfs:label>
    <rdfs:comment>The etag for this rule.
If this is provided on update, the request will succeed if and only if it
matches the server-computed value, and will fail with an ABORTED error
otherwise.
Populated in BASIC view and FULL view.</rdfs:comment>
    <rdfs:domain rdf:resource="http://example.org/onto/class/google_chronicle_rule"/>
    <rdfs:range rdf:resource="http://www.w3.org/2001/XMLSchema#string"/>
  </owl:DatatypeProperty>
  <owl:DatatypeProperty rdf:about="http://example.org/onto/prop/google_chronicle_rule_id">
    <rdfs:label>id</rdfs:label>
    <rdfs:domain rdf:resource="http://example.org/onto/class/google_chronicle_rule"/>
    <rdfs:range rdf:resource="http://www.w3.org/2001/XMLSchema#string"/>
  </owl:DatatypeProperty>
  <owl:DatatypeProperty rdf:about="http://example.org/onto/prop/google_chronicle_rule_instance">
    <rdfs:label>instance</rdfs:label>
    <rdfs:comment>The unique identifier for the Chronicle instance, which is the same as the customer ID.</rdfs:comment>
    <rdfs:domain rdf:resource="http://example.org/onto/class/google_chronicle_rule"/>
    <rdfs:range rdf:resource="http://www.w3.org/2001/XMLSchema#string"/>
  </owl:DatatypeProperty>
  <owl:DatatypeProperty rdf:about="http://example.org/onto/prop/google_chronicle_rule_location">
    <rdfs:label>location</rdfs:label>
    <rdfs:comment>The location of the resource. This is the geographical region where the Chronicle instance resides, such as "us" or "europe-west2".</rdfs:comment>
    <rdfs:domain rdf:resource="http://example.org/onto/class/google_chronicle_rule"/>
    <rdfs:range rdf:resource="http://www.w3.org/2001/XMLSchema#string"/>
  </owl:DatatypeProperty>
  <owl:DatatypeProperty rdf:about="http://example.org/onto/prop/google_chronicle_rule_metadata">
    <rdfs:label>metadata</rdfs:label>
    <rdfs:comment>Output only. Additional metadata specified in the meta section of text.
Populated in FULL view.</rdfs:comment>
    <rdfs:domain rdf:resource="http://example.org/onto/class/google_chronicle_rule"/>
    <rdfs:range rdf:resource="http://www.w3.org/2001/XMLSchema#string"/>
  </owl:DatatypeProperty>
  <owl:DatatypeProperty rdf:about="http://example.org/onto/prop/google_chronicle_rule_name">
    <rdfs:label>name</rdfs:label>
    <rdfs:comment>Full resource name for the rule. This unique identifier is generated using values provided for the URL parameters.
Format:
projects/{project}/locations/{location}/instances/{instance}/rules/{rule}</rdfs:comment>
    <rdfs:domain rdf:resource="http://example.org/onto/class/google_chronicle_rule"/>
    <rdfs:range rdf:resource="http://www.w3.org/2001/XMLSchema#string"/>
  </owl:DatatypeProperty>
  <owl:DatatypeProperty rdf:about="http://example.org/onto/prop/google_chronicle_rule_near_real_time_live_rule_eligible">
    <rdfs:label>near_real_time_live_rule_eligible</rdfs:label>
    <rdfs:comment>Output only. Indicate the rule can run in near real time live rule.
If this is true, the rule uses the near real time live rule when the run
frequency is set to LIVE.</rdfs:comment>
    <rdfs:domain rdf:resource="http://example.org/onto/class/google_chronicle_rule"/>
    <rdfs:range rdf:resource="http://www.w3.org/2001/XMLSchema#string"/>
  </owl:DatatypeProperty>
  <owl:DatatypeProperty rdf:about="http://example.org/onto/prop/google_chronicle_rule_project">
    <rdfs:label>project</rdfs:label>
    <rdfs:domain rdf:resource="http://example.org/onto/class/google_chronicle_rule"/>
    <rdfs:range rdf:resource="http://www.w3.org/2001/XMLSchema#string"/>
  </owl:DatatypeProperty>
  <owl:DatatypeProperty rdf:about="http://example.org/onto/prop/google_chronicle_rule_reference_lists">
    <rdfs:label>reference_lists</rdfs:label>
    <rdfs:comment>Output only. Resource names of the reference lists used in this rule.
Populated in FULL view.</rdfs:comment>
    <rdfs:domain rdf:resource="http://example.org/onto/class/google_chronicle_rule"/>
    <rdfs:range rdf:resource="http://www.w3.org/2001/XMLSchema#string"/>
  </owl:DatatypeProperty>
  <owl:DatatypeProperty rdf:about="http://example.org/onto/prop/google_chronicle_rule_revision_create_time">
    <rdfs:label>revision_create_time</rdfs:label>
    <rdfs:comment>Output only. The timestamp of when the rule revision was created.
Populated in FULL, REVISION_METADATA_ONLY views.</rdfs:comment>
    <rdfs:domain rdf:resource="http://example.org/onto/class/google_chronicle_rule"/>
    <rdfs:range rdf:resource="http://www.w3.org/2001/XMLSchema#string"/>
  </owl:DatatypeProperty>
  <owl:DatatypeProperty rdf:about="http://example.org/onto/prop/google_chronicle_rule_revision_id">
    <rdfs:label>revision_id</rdfs:label>
    <rdfs:comment>Output only. The revision ID of the rule.
A new revision is created whenever the rule text is changed in any way.
Format: v_{10 digits}_{9 digits}
Populated in REVISION_METADATA_ONLY view and FULL view.</rdfs:comment>
    <rdfs:domain rdf:resource="http://example.org/onto/class/google_chronicle_rule"/>
    <rdfs:range rdf:resource="http://www.w3.org/2001/XMLSchema#string"/>
  </owl:DatatypeProperty>
  <owl:DatatypeProperty rdf:about="http://example.org/onto/prop/google_chronicle_rule_rule_id">
    <rdfs:label>rule_id</rdfs:label>
    <rdfs:comment>Rule Id is the ID of the Rule.</rdfs:comment>
    <rdfs:domain rdf:resource="http://example.org/onto/class/google_chronicle_rule"/>
    <rdfs:range rdf:resource="http://www.w3.org/2001/XMLSchema#string"/>
  </owl:DatatypeProperty>
  <owl:DatatypeProperty rdf:about="http://example.org/onto/prop/google_chronicle_rule_scope">
    <rdfs:label>scope</rdfs:label>
    <rdfs:comment>Resource name of the DataAccessScope bound to this rule.
Populated in BASIC view and FULL view.
If reference lists are used in the rule, validations will be performed
against this scope to ensure that the reference lists are compatible with
both the user's and the rule's scopes.
The scope should be in the format:
"projects/{project}/locations/{location}/instances/{instance}/dataAccessScopes/{scope}".</rdfs:comment>
    <rdfs:domain rdf:resource="http://example.org/onto/class/google_chronicle_rule"/>
    <rdfs:range rdf:resource="http://www.w3.org/2001/XMLSchema#string"/>
  </owl:DatatypeProperty>
  <owl:DatatypeProperty rdf:about="http://example.org/onto/prop/google_chronicle_rule_severity">
    <rdfs:label>severity</rdfs:label>
    <rdfs:comment>Severity represents the severity level of the rule.</rdfs:comment>
    <rdfs:domain rdf:resource="http://example.org/onto/class/google_chronicle_rule"/>
    <rdfs:range rdf:resource="http://www.w3.org/2001/XMLSchema#string"/>
  </owl:DatatypeProperty>
  <owl:DatatypeProperty rdf:about="http://example.org/onto/prop/google_chronicle_rule_text">
    <rdfs:label>text</rdfs:label>
    <rdfs:comment>The YARA-L content of the rule.
Populated in FULL view.</rdfs:comment>
    <rdfs:domain rdf:resource="http://example.org/onto/class/google_chronicle_rule"/>
    <rdfs:range rdf:resource="http://www.w3.org/2001/XMLSchema#string"/>
  </owl:DatatypeProperty>
  <owl:DatatypeProperty rdf:about="http://example.org/onto/prop/google_chronicle_rule_type">
    <rdfs:label>type</rdfs:label>
    <rdfs:comment>Possible values:
RULE_TYPE_UNSPECIFIED
SINGLE_EVENT
MULTI_EVENT</rdfs:comment>
    <rdfs:domain rdf:resource="http://example.org/onto/class/google_chronicle_rule"/>
    <rdfs:range rdf:resource="http://www.w3.org/2001/XMLSchema#string"/>
  </owl:DatatypeProperty>
  <owl:DatatypeProperty rdf:about="http://example.org/onto/prop/google_chronicle_rule_create">
    <rdfs:label>create</rdfs:label>
    <rdfs:domain rdf:resource="http://example.org/onto/class/google_chronicle_rule"/>
    <rdfs:range rdf:resource="http://www.w3.org/2001/XMLSchema#string"/>
  </owl:DatatypeProperty>
  <owl:DatatypeProperty rdf:about="http://example.org/onto/prop/google_chronicle_rule_delete">
    <rdfs:label>delete</rdfs:label>
    <rdfs:domain rdf:resource="http://example.org/onto/class/google_chronicle_rule"/>
    <rdfs:range rdf:resource="http://www.w3.org/2001/XMLSchema#string"/>
  </owl:DatatypeProperty>
  <owl:DatatypeProperty rdf:about="http://example.org/onto/prop/google_chronicle_rule_update">
    <rdfs:label>update</rdfs:label>
    <rdfs:domain rdf:resource="http://example.org/onto/class/google_chronicle_rule"/>
    <rdfs:range rdf:resource="http://www.w3.org/2001/XMLSchema#string"/>
  </owl:DatatypeProperty>
</rdf:RDF>
