<?xml version="1.0" encoding="UTF-8"?>
<rdf:RDF
  xmlns:rdf="http://www.w3.org/1999/02/22-rdf-syntax-ns#"
  xmlns:rdfs="http://www.w3.org/2000/01/rdf-schema#"
  xmlns:owl="http://www.w3.org/2002/07/owl#"
  xmlns:xsd="http://www.w3.org/2001/XMLSchema#"
  xml:base="http://example.org/onto/">
  <owl:Class rdf:about="http://example.org/onto/class/google_healthcare_pipeline_job">
    <rdfs:label>google_healthcare_pipeline_job</rdfs:label>
    <rdfs:comment>#
#     ***     AUTO GENERATED CODE    ***    Type: MMv1     ***
#
# ----------------------------------------------------------------------------
#
#     This code is generated by Magic Modules using the following:
#
#     Configuration: https:#github.com/GoogleCloudPlatform/magic-modules/tree/main/mmv1/products/healthcare/PipelineJob.yaml
#     Template:      https:#github.com/GoogleCloudPlatform/magic-modules/tree/main/mmv1/templates/terraform/resource.html.markdown.tmpl
#
#     DO NOT EDIT this file directly. Any changes made to this file will be
#     overwritten during the next generation cycle.
#
# ----------------------------------------------------------------------------
subcategory: "Cloud Healthcare"
description: |-
  PipelineJobs are Long Running Operations on Healthcare API to Map or Reconcile
  incoming data into FHIR format
---</rdfs:comment>
  </owl:Class>
  <owl:DatatypeProperty rdf:about="http://example.org/onto/prop/google_healthcare_pipeline_job_dataset">
    <rdfs:label>dataset</rdfs:label>
    <rdfs:comment>Healthcare Dataset under which the Pipeline Job is to run</rdfs:comment>
    <rdfs:domain rdf:resource="http://example.org/onto/class/google_healthcare_pipeline_job"/>
    <rdfs:range rdf:resource="http://www.w3.org/2001/XMLSchema#string"/>
  </owl:DatatypeProperty>
  <owl:DatatypeProperty rdf:about="http://example.org/onto/prop/google_healthcare_pipeline_job_disable_lineage">
    <rdfs:label>disable_lineage</rdfs:label>
    <rdfs:comment>If true, disables writing lineage for the pipeline.</rdfs:comment>
    <rdfs:domain rdf:resource="http://example.org/onto/class/google_healthcare_pipeline_job"/>
    <rdfs:range rdf:resource="http://www.w3.org/2001/XMLSchema#string"/>
  </owl:DatatypeProperty>
  <owl:DatatypeProperty rdf:about="http://example.org/onto/prop/google_healthcare_pipeline_job_effective_labels">
    <rdfs:label>effective_labels</rdfs:label>
    <rdfs:comment>All of labels (key/value pairs) present on the resource in GCP, including the labels configured through Terraform, other clients and services.</rdfs:comment>
    <rdfs:domain rdf:resource="http://example.org/onto/class/google_healthcare_pipeline_job"/>
    <rdfs:range rdf:resource="http://www.w3.org/2001/XMLSchema#string"/>
  </owl:DatatypeProperty>
  <owl:DatatypeProperty rdf:about="http://example.org/onto/prop/google_healthcare_pipeline_job_id">
    <rdfs:label>id</rdfs:label>
    <rdfs:domain rdf:resource="http://example.org/onto/class/google_healthcare_pipeline_job"/>
    <rdfs:range rdf:resource="http://www.w3.org/2001/XMLSchema#string"/>
  </owl:DatatypeProperty>
  <owl:DatatypeProperty rdf:about="http://example.org/onto/prop/google_healthcare_pipeline_job_labels">
    <rdfs:label>labels</rdfs:label>
    <rdfs:comment>User-supplied key-value pairs used to organize Pipeline Jobs.
Label keys must be between 1 and 63 characters long, have a UTF-8 encoding of
maximum 128 bytes, and must conform to the following PCRE regular expression:
[\p{Ll}\p{Lo}][\p{Ll}\p{Lo}\p{N}_-]{0,62}
Label values are optional, must be between 1 and 63 characters long, have a
UTF-8 encoding of maximum 128 bytes, and must conform to the following PCRE
regular expression: [\p{Ll}\p{Lo}\p{N}_-]{0,63}
No more than 64 labels can be associated with a given pipeline.
An object containing a list of "key": value pairs.
Example: { "name": "wrench", "mass": "1.3kg", "count": "3" }.


**Note**: This field is non-authoritative, and will only manage the labels present in your configuration.
Please refer to the field 'effective_labels' for all of the labels present on the resource.</rdfs:comment>
    <rdfs:domain rdf:resource="http://example.org/onto/class/google_healthcare_pipeline_job"/>
    <rdfs:range rdf:resource="http://www.w3.org/2001/XMLSchema#string"/>
  </owl:DatatypeProperty>
  <owl:DatatypeProperty rdf:about="http://example.org/onto/prop/google_healthcare_pipeline_job_location">
    <rdfs:label>location</rdfs:label>
    <rdfs:comment>Location where the Pipeline Job is to run</rdfs:comment>
    <rdfs:domain rdf:resource="http://example.org/onto/class/google_healthcare_pipeline_job"/>
    <rdfs:range rdf:resource="http://www.w3.org/2001/XMLSchema#string"/>
  </owl:DatatypeProperty>
  <owl:DatatypeProperty rdf:about="http://example.org/onto/prop/google_healthcare_pipeline_job_name">
    <rdfs:label>name</rdfs:label>
    <rdfs:comment>Specifies the name of the pipeline job. This field is user-assigned.</rdfs:comment>
    <rdfs:domain rdf:resource="http://example.org/onto/class/google_healthcare_pipeline_job"/>
    <rdfs:range rdf:resource="http://www.w3.org/2001/XMLSchema#string"/>
  </owl:DatatypeProperty>
  <owl:DatatypeProperty rdf:about="http://example.org/onto/prop/google_healthcare_pipeline_job_self_link">
    <rdfs:label>self_link</rdfs:label>
    <rdfs:comment>The fully qualified name of this dataset</rdfs:comment>
    <rdfs:domain rdf:resource="http://example.org/onto/class/google_healthcare_pipeline_job"/>
    <rdfs:range rdf:resource="http://www.w3.org/2001/XMLSchema#string"/>
  </owl:DatatypeProperty>
  <owl:DatatypeProperty rdf:about="http://example.org/onto/prop/google_healthcare_pipeline_job_terraform_labels">
    <rdfs:label>terraform_labels</rdfs:label>
    <rdfs:comment>The combination of labels configured directly on the resource
 and default labels configured on the provider.</rdfs:comment>
    <rdfs:domain rdf:resource="http://example.org/onto/class/google_healthcare_pipeline_job"/>
    <rdfs:range rdf:resource="http://www.w3.org/2001/XMLSchema#string"/>
  </owl:DatatypeProperty>
  <owl:DatatypeProperty rdf:about="http://example.org/onto/prop/google_healthcare_pipeline_job_mapping_pipeline_job">
    <rdfs:label>mapping_pipeline_job</rdfs:label>
    <rdfs:comment>Specifies the mapping pipeline job to backfill, the name format
should follow: projects/{projectId}/locations/{locationId}/datasets/{datasetId}/pipelineJobs/{pipelineJobId}.</rdfs:comment>
    <rdfs:domain rdf:resource="http://example.org/onto/class/google_healthcare_pipeline_job"/>
    <rdfs:range rdf:resource="http://www.w3.org/2001/XMLSchema#string"/>
  </owl:DatatypeProperty>
  <owl:DatatypeProperty rdf:about="http://example.org/onto/prop/google_healthcare_pipeline_job_fhir_store_destination">
    <rdfs:label>fhir_store_destination</rdfs:label>
    <rdfs:comment>If set, the mapping pipeline will write snapshots to this
FHIR store without assigning stable IDs. You must
grant your pipeline project's Cloud Healthcare Service
Agent serviceaccount healthcare.fhirResources.executeBundle
and healthcare.fhirResources.create permissions on the
destination store. The destination store must set
[disableReferentialIntegrity][FhirStore.disable_referential_integrity]
to true. The destination store must use FHIR version R4.
Format: project/{projectID}/locations/{locationID}/datasets/{datasetName}/fhirStores/{fhirStoreID}.</rdfs:comment>
    <rdfs:domain rdf:resource="http://example.org/onto/class/google_healthcare_pipeline_job"/>
    <rdfs:range rdf:resource="http://www.w3.org/2001/XMLSchema#string"/>
  </owl:DatatypeProperty>
  <owl:DatatypeProperty rdf:about="http://example.org/onto/prop/google_healthcare_pipeline_job_reconciliation_destination">
    <rdfs:label>reconciliation_destination</rdfs:label>
    <rdfs:comment>If set to true, a mapping pipeline will send output snapshots
to the reconciliation pipeline in its dataset. A reconciliation
pipeline must exist in this dataset before a mapping pipeline
with a reconciliation destination can be created.</rdfs:comment>
    <rdfs:domain rdf:resource="http://example.org/onto/class/google_healthcare_pipeline_job"/>
    <rdfs:range rdf:resource="http://www.w3.org/2001/XMLSchema#string"/>
  </owl:DatatypeProperty>
  <owl:DatatypeProperty rdf:about="http://example.org/onto/prop/google_healthcare_pipeline_job_description">
    <rdfs:label>description</rdfs:label>
    <rdfs:comment>Describes the streaming FHIR data source.</rdfs:comment>
    <rdfs:domain rdf:resource="http://example.org/onto/class/google_healthcare_pipeline_job"/>
    <rdfs:range rdf:resource="http://www.w3.org/2001/XMLSchema#string"/>
  </owl:DatatypeProperty>
  <owl:DatatypeProperty rdf:about="http://example.org/onto/prop/google_healthcare_pipeline_job_fhir_store">
    <rdfs:label>fhir_store</rdfs:label>
    <rdfs:comment>The path to the FHIR store in the format projects/{projectId}/locations/{locationId}/datasets/{datasetId}/fhirStores/{fhirStoreId}.</rdfs:comment>
    <rdfs:domain rdf:resource="http://example.org/onto/class/google_healthcare_pipeline_job"/>
    <rdfs:range rdf:resource="http://www.w3.org/2001/XMLSchema#string"/>
  </owl:DatatypeProperty>
  <owl:DatatypeProperty rdf:about="http://example.org/onto/prop/google_healthcare_pipeline_job_description">
    <rdfs:label>description</rdfs:label>
    <rdfs:comment>Describes the mapping configuration.</rdfs:comment>
    <rdfs:domain rdf:resource="http://example.org/onto/class/google_healthcare_pipeline_job"/>
    <rdfs:range rdf:resource="http://www.w3.org/2001/XMLSchema#string"/>
  </owl:DatatypeProperty>
  <owl:DatatypeProperty rdf:about="http://example.org/onto/prop/google_healthcare_pipeline_job_import_uri_prefix">
    <rdfs:label>import_uri_prefix</rdfs:label>
    <rdfs:comment>Directory path where all the Whistle files are located.
Example: gs://{bucket-id}/{path/to/import-root/dir}</rdfs:comment>
    <rdfs:domain rdf:resource="http://example.org/onto/class/google_healthcare_pipeline_job"/>
    <rdfs:range rdf:resource="http://www.w3.org/2001/XMLSchema#string"/>
  </owl:DatatypeProperty>
  <owl:DatatypeProperty rdf:about="http://example.org/onto/prop/google_healthcare_pipeline_job_uri">
    <rdfs:label>uri</rdfs:label>
    <rdfs:comment>Main configuration file which has the entrypoint or the root function.
Example: gs://{bucket-id}/{path/to/import-root/dir}/entrypoint-file-name.wstl.</rdfs:comment>
    <rdfs:domain rdf:resource="http://example.org/onto/class/google_healthcare_pipeline_job"/>
    <rdfs:range rdf:resource="http://www.w3.org/2001/XMLSchema#string"/>
  </owl:DatatypeProperty>
  <owl:DatatypeProperty rdf:about="http://example.org/onto/prop/google_healthcare_pipeline_job_fhir_store_destination">
    <rdfs:label>fhir_store_destination</rdfs:label>
    <rdfs:comment>The harmonized FHIR store to write harmonized FHIR resources to,
in the format of: project/{projectID}/locations/{locationID}/datasets/{datasetName}/fhirStores/{id}</rdfs:comment>
    <rdfs:domain rdf:resource="http://example.org/onto/class/google_healthcare_pipeline_job"/>
    <rdfs:range rdf:resource="http://www.w3.org/2001/XMLSchema#string"/>
  </owl:DatatypeProperty>
  <owl:DatatypeProperty rdf:about="http://example.org/onto/prop/google_healthcare_pipeline_job_matching_uri_prefix">
    <rdfs:label>matching_uri_prefix</rdfs:label>
    <rdfs:comment>Specifies the top level directory of the matching configs used
in all mapping pipelines, which extract properties for resources
to be matched on.
Example: gs://{bucket-id}/{path/to/matching/configs}</rdfs:comment>
    <rdfs:domain rdf:resource="http://example.org/onto/class/google_healthcare_pipeline_job"/>
    <rdfs:range rdf:resource="http://www.w3.org/2001/XMLSchema#string"/>
  </owl:DatatypeProperty>
  <owl:DatatypeProperty rdf:about="http://example.org/onto/prop/google_healthcare_pipeline_job_description">
    <rdfs:label>description</rdfs:label>
    <rdfs:comment>Describes the mapping configuration.</rdfs:comment>
    <rdfs:domain rdf:resource="http://example.org/onto/class/google_healthcare_pipeline_job"/>
    <rdfs:range rdf:resource="http://www.w3.org/2001/XMLSchema#string"/>
  </owl:DatatypeProperty>
  <owl:DatatypeProperty rdf:about="http://example.org/onto/prop/google_healthcare_pipeline_job_import_uri_prefix">
    <rdfs:label>import_uri_prefix</rdfs:label>
    <rdfs:comment>Directory path where all the Whistle files are located.
Example: gs://{bucket-id}/{path/to/import-root/dir}</rdfs:comment>
    <rdfs:domain rdf:resource="http://example.org/onto/class/google_healthcare_pipeline_job"/>
    <rdfs:range rdf:resource="http://www.w3.org/2001/XMLSchema#string"/>
  </owl:DatatypeProperty>
  <owl:DatatypeProperty rdf:about="http://example.org/onto/prop/google_healthcare_pipeline_job_uri">
    <rdfs:label>uri</rdfs:label>
    <rdfs:comment>Main configuration file which has the entrypoint or the root function.
Example: gs://{bucket-id}/{path/to/import-root/dir}/entrypoint-file-name.wstl.</rdfs:comment>
    <rdfs:domain rdf:resource="http://example.org/onto/class/google_healthcare_pipeline_job"/>
    <rdfs:range rdf:resource="http://www.w3.org/2001/XMLSchema#string"/>
  </owl:DatatypeProperty>
  <owl:DatatypeProperty rdf:about="http://example.org/onto/prop/google_healthcare_pipeline_job_create">
    <rdfs:label>create</rdfs:label>
    <rdfs:domain rdf:resource="http://example.org/onto/class/google_healthcare_pipeline_job"/>
    <rdfs:range rdf:resource="http://www.w3.org/2001/XMLSchema#string"/>
  </owl:DatatypeProperty>
  <owl:DatatypeProperty rdf:about="http://example.org/onto/prop/google_healthcare_pipeline_job_delete">
    <rdfs:label>delete</rdfs:label>
    <rdfs:domain rdf:resource="http://example.org/onto/class/google_healthcare_pipeline_job"/>
    <rdfs:range rdf:resource="http://www.w3.org/2001/XMLSchema#string"/>
  </owl:DatatypeProperty>
  <owl:DatatypeProperty rdf:about="http://example.org/onto/prop/google_healthcare_pipeline_job_update">
    <rdfs:label>update</rdfs:label>
    <rdfs:domain rdf:resource="http://example.org/onto/class/google_healthcare_pipeline_job"/>
    <rdfs:range rdf:resource="http://www.w3.org/2001/XMLSchema#string"/>
  </owl:DatatypeProperty>
</rdf:RDF>
