<?xml version="1.0" encoding="UTF-8"?>
<rdf:RDF
  xmlns:rdf="http://www.w3.org/1999/02/22-rdf-syntax-ns#"
  xmlns:rdfs="http://www.w3.org/2000/01/rdf-schema#"
  xmlns:owl="http://www.w3.org/2002/07/owl#"
  xmlns:xsd="http://www.w3.org/2001/XMLSchema#"
  xml:base="http://example.org/onto/">
  <owl:Class rdf:about="http://example.org/onto/class/google_storage_bucket">
    <rdfs:label>google_storage_bucket</rdfs:label>
    <rdfs:comment>#
#     ***     AUTO GENERATED CODE    ***    Type: Handwritten     ***
#
# ----------------------------------------------------------------------------
#
#     This code is generated by Magic Modules using the following:
#
#     Source file: https://github.com/GoogleCloudPlatform/magic-modules/tree/main/mmv1/third_party/terraform/website/docs/r/storage_bucket.html.markdown
#
#     DO NOT EDIT this file directly. Any changes made to this file will be
#     overwritten during the next generation cycle.
#
# ----------------------------------------------------------------------------
subcategory: "Cloud Storage"
description: |-
  Creates a new bucket in Google Cloud Storage.
---</rdfs:comment>
  </owl:Class>
  <owl:DatatypeProperty rdf:about="http://example.org/onto/prop/google_storage_bucket_default_event_based_hold">
    <rdfs:label>default_event_based_hold</rdfs:label>
    <rdfs:comment>Whether or not to automatically apply an eventBasedHold to new objects added to the bucket.</rdfs:comment>
    <rdfs:domain rdf:resource="http://example.org/onto/class/google_storage_bucket"/>
    <rdfs:range rdf:resource="http://www.w3.org/2001/XMLSchema#string"/>
  </owl:DatatypeProperty>
  <owl:DatatypeProperty rdf:about="http://example.org/onto/prop/google_storage_bucket_effective_labels">
    <rdfs:label>effective_labels</rdfs:label>
    <rdfs:comment>All of labels (key/value pairs) present on the resource in GCP, including the labels configured through Terraform, other clients and services.</rdfs:comment>
    <rdfs:domain rdf:resource="http://example.org/onto/class/google_storage_bucket"/>
    <rdfs:range rdf:resource="http://www.w3.org/2001/XMLSchema#string"/>
  </owl:DatatypeProperty>
  <owl:DatatypeProperty rdf:about="http://example.org/onto/prop/google_storage_bucket_enable_object_retention">
    <rdfs:label>enable_object_retention</rdfs:label>
    <rdfs:comment>Enables each object in the bucket to have its own retention policy, which prevents deletion until stored for a specific length of time.</rdfs:comment>
    <rdfs:domain rdf:resource="http://example.org/onto/class/google_storage_bucket"/>
    <rdfs:range rdf:resource="http://www.w3.org/2001/XMLSchema#string"/>
  </owl:DatatypeProperty>
  <owl:DatatypeProperty rdf:about="http://example.org/onto/prop/google_storage_bucket_force_destroy">
    <rdfs:label>force_destroy</rdfs:label>
    <rdfs:comment>When deleting a bucket, this boolean option will delete all contained objects, or anywhereCaches (if any). If you try to delete a bucket that contains objects or anywhereCaches, Terraform will fail that run, deleting anywhereCaches may take 80 minutes to complete.</rdfs:comment>
    <rdfs:domain rdf:resource="http://example.org/onto/class/google_storage_bucket"/>
    <rdfs:range rdf:resource="http://www.w3.org/2001/XMLSchema#string"/>
  </owl:DatatypeProperty>
  <owl:DatatypeProperty rdf:about="http://example.org/onto/prop/google_storage_bucket_id">
    <rdfs:label>id</rdfs:label>
    <rdfs:domain rdf:resource="http://example.org/onto/class/google_storage_bucket"/>
    <rdfs:range rdf:resource="http://www.w3.org/2001/XMLSchema#string"/>
  </owl:DatatypeProperty>
  <owl:DatatypeProperty rdf:about="http://example.org/onto/prop/google_storage_bucket_labels">
    <rdfs:label>labels</rdfs:label>
    <rdfs:comment>A set of key/value label pairs to assign to the bucket.</rdfs:comment>
    <rdfs:domain rdf:resource="http://example.org/onto/class/google_storage_bucket"/>
    <rdfs:range rdf:resource="http://www.w3.org/2001/XMLSchema#string"/>
  </owl:DatatypeProperty>
  <owl:DatatypeProperty rdf:about="http://example.org/onto/prop/google_storage_bucket_location">
    <rdfs:label>location</rdfs:label>
    <rdfs:comment>The Google Cloud Storage location or region.</rdfs:comment>
    <rdfs:domain rdf:resource="http://example.org/onto/class/google_storage_bucket"/>
    <rdfs:range rdf:resource="http://www.w3.org/2001/XMLSchema#string"/>
  </owl:DatatypeProperty>
  <owl:DatatypeProperty rdf:about="http://example.org/onto/prop/google_storage_bucket_name">
    <rdfs:label>name</rdfs:label>
    <rdfs:comment>The name of the bucket.</rdfs:comment>
    <rdfs:domain rdf:resource="http://example.org/onto/class/google_storage_bucket"/>
    <rdfs:range rdf:resource="http://www.w3.org/2001/XMLSchema#string"/>
  </owl:DatatypeProperty>
  <owl:DatatypeProperty rdf:about="http://example.org/onto/prop/google_storage_bucket_project">
    <rdfs:label>project</rdfs:label>
    <rdfs:comment>The ID of the project in which the resource belongs. If it is not provided, the provider project is used.</rdfs:comment>
    <rdfs:domain rdf:resource="http://example.org/onto/class/google_storage_bucket"/>
    <rdfs:range rdf:resource="http://www.w3.org/2001/XMLSchema#string"/>
  </owl:DatatypeProperty>
  <owl:DatatypeProperty rdf:about="http://example.org/onto/prop/google_storage_bucket_project_number">
    <rdfs:label>project_number</rdfs:label>
    <rdfs:comment>The project number of the project in which the resource belongs.</rdfs:comment>
    <rdfs:domain rdf:resource="http://example.org/onto/class/google_storage_bucket"/>
    <rdfs:range rdf:resource="http://www.w3.org/2001/XMLSchema#string"/>
  </owl:DatatypeProperty>
  <owl:DatatypeProperty rdf:about="http://example.org/onto/prop/google_storage_bucket_public_access_prevention">
    <rdfs:label>public_access_prevention</rdfs:label>
    <rdfs:comment>Prevents public access to a bucket.</rdfs:comment>
    <rdfs:domain rdf:resource="http://example.org/onto/class/google_storage_bucket"/>
    <rdfs:range rdf:resource="http://www.w3.org/2001/XMLSchema#string"/>
  </owl:DatatypeProperty>
  <owl:DatatypeProperty rdf:about="http://example.org/onto/prop/google_storage_bucket_requester_pays">
    <rdfs:label>requester_pays</rdfs:label>
    <rdfs:comment>Enables Requester Pays on a storage bucket.</rdfs:comment>
    <rdfs:domain rdf:resource="http://example.org/onto/class/google_storage_bucket"/>
    <rdfs:range rdf:resource="http://www.w3.org/2001/XMLSchema#string"/>
  </owl:DatatypeProperty>
  <owl:DatatypeProperty rdf:about="http://example.org/onto/prop/google_storage_bucket_rpo">
    <rdfs:label>rpo</rdfs:label>
    <rdfs:comment>Specifies the RPO setting of bucket. If set 'ASYNC_TURBO', The Turbo Replication will be enabled for the dual-region bucket. Value 'DEFAULT' will set RPO setting to default. Turbo Replication is only for buckets in dual-regions.See the docs for more details.</rdfs:comment>
    <rdfs:domain rdf:resource="http://example.org/onto/class/google_storage_bucket"/>
    <rdfs:range rdf:resource="http://www.w3.org/2001/XMLSchema#string"/>
  </owl:DatatypeProperty>
  <owl:DatatypeProperty rdf:about="http://example.org/onto/prop/google_storage_bucket_self_link">
    <rdfs:label>self_link</rdfs:label>
    <rdfs:comment>The URI of the created resource.</rdfs:comment>
    <rdfs:domain rdf:resource="http://example.org/onto/class/google_storage_bucket"/>
    <rdfs:range rdf:resource="http://www.w3.org/2001/XMLSchema#string"/>
  </owl:DatatypeProperty>
  <owl:DatatypeProperty rdf:about="http://example.org/onto/prop/google_storage_bucket_storage_class">
    <rdfs:label>storage_class</rdfs:label>
    <rdfs:comment>The Storage Class of the new bucket. Supported values include: STANDARD, MULTI_REGIONAL, REGIONAL, NEARLINE, COLDLINE, ARCHIVE.</rdfs:comment>
    <rdfs:domain rdf:resource="http://example.org/onto/class/google_storage_bucket"/>
    <rdfs:range rdf:resource="http://www.w3.org/2001/XMLSchema#string"/>
  </owl:DatatypeProperty>
  <owl:DatatypeProperty rdf:about="http://example.org/onto/prop/google_storage_bucket_terraform_labels">
    <rdfs:label>terraform_labels</rdfs:label>
    <rdfs:comment>The combination of labels configured directly on the resource and default labels configured on the provider.</rdfs:comment>
    <rdfs:domain rdf:resource="http://example.org/onto/class/google_storage_bucket"/>
    <rdfs:range rdf:resource="http://www.w3.org/2001/XMLSchema#string"/>
  </owl:DatatypeProperty>
  <owl:DatatypeProperty rdf:about="http://example.org/onto/prop/google_storage_bucket_time_created">
    <rdfs:label>time_created</rdfs:label>
    <rdfs:comment>The creation time of the bucket in RFC 3339 format.</rdfs:comment>
    <rdfs:domain rdf:resource="http://example.org/onto/class/google_storage_bucket"/>
    <rdfs:range rdf:resource="http://www.w3.org/2001/XMLSchema#string"/>
  </owl:DatatypeProperty>
  <owl:DatatypeProperty rdf:about="http://example.org/onto/prop/google_storage_bucket_uniform_bucket_level_access">
    <rdfs:label>uniform_bucket_level_access</rdfs:label>
    <rdfs:comment>Enables uniform bucket-level access on a bucket.</rdfs:comment>
    <rdfs:domain rdf:resource="http://example.org/onto/class/google_storage_bucket"/>
    <rdfs:range rdf:resource="http://www.w3.org/2001/XMLSchema#string"/>
  </owl:DatatypeProperty>
  <owl:DatatypeProperty rdf:about="http://example.org/onto/prop/google_storage_bucket_updated">
    <rdfs:label>updated</rdfs:label>
    <rdfs:comment>The time at which the bucket's metadata or IAM policy was last updated, in RFC 3339 format.</rdfs:comment>
    <rdfs:domain rdf:resource="http://example.org/onto/class/google_storage_bucket"/>
    <rdfs:range rdf:resource="http://www.w3.org/2001/XMLSchema#string"/>
  </owl:DatatypeProperty>
  <owl:DatatypeProperty rdf:about="http://example.org/onto/prop/google_storage_bucket_url">
    <rdfs:label>url</rdfs:label>
    <rdfs:comment>The base URL of the bucket, in the format gs://<bucket-name>.</rdfs:comment>
    <rdfs:domain rdf:resource="http://example.org/onto/class/google_storage_bucket"/>
    <rdfs:range rdf:resource="http://www.w3.org/2001/XMLSchema#string"/>
  </owl:DatatypeProperty>
  <owl:DatatypeProperty rdf:about="http://example.org/onto/prop/google_storage_bucket_enabled">
    <rdfs:label>enabled</rdfs:label>
    <rdfs:comment>While set to true, autoclass automatically transitions objects in your bucket to appropriate storage classes based on each object's access pattern.</rdfs:comment>
    <rdfs:domain rdf:resource="http://example.org/onto/class/google_storage_bucket"/>
    <rdfs:range rdf:resource="http://www.w3.org/2001/XMLSchema#string"/>
  </owl:DatatypeProperty>
  <owl:DatatypeProperty rdf:about="http://example.org/onto/prop/google_storage_bucket_terminal_storage_class">
    <rdfs:label>terminal_storage_class</rdfs:label>
    <rdfs:comment>The storage class that objects in the bucket eventually transition to if they are not read for a certain length of time. Supported values include: NEARLINE, ARCHIVE.</rdfs:comment>
    <rdfs:domain rdf:resource="http://example.org/onto/class/google_storage_bucket"/>
    <rdfs:range rdf:resource="http://www.w3.org/2001/XMLSchema#string"/>
  </owl:DatatypeProperty>
  <owl:DatatypeProperty rdf:about="http://example.org/onto/prop/google_storage_bucket_max_age_seconds">
    <rdfs:label>max_age_seconds</rdfs:label>
    <rdfs:comment>The value, in seconds, to return in the Access-Control-Max-Age header used in preflight responses.</rdfs:comment>
    <rdfs:domain rdf:resource="http://example.org/onto/class/google_storage_bucket"/>
    <rdfs:range rdf:resource="http://www.w3.org/2001/XMLSchema#string"/>
  </owl:DatatypeProperty>
  <owl:DatatypeProperty rdf:about="http://example.org/onto/prop/google_storage_bucket_method">
    <rdfs:label>method</rdfs:label>
    <rdfs:comment>The list of HTTP methods on which to include CORS response headers, (GET, OPTIONS, POST, etc) Note: "*" is permitted in the list of methods, and means "any method".</rdfs:comment>
    <rdfs:domain rdf:resource="http://example.org/onto/class/google_storage_bucket"/>
    <rdfs:range rdf:resource="http://www.w3.org/2001/XMLSchema#string"/>
  </owl:DatatypeProperty>
  <owl:DatatypeProperty rdf:about="http://example.org/onto/prop/google_storage_bucket_origin">
    <rdfs:label>origin</rdfs:label>
    <rdfs:comment>The list of Origins eligible to receive CORS response headers. Note: "*" is permitted in the list of origins, and means "any Origin".</rdfs:comment>
    <rdfs:domain rdf:resource="http://example.org/onto/class/google_storage_bucket"/>
    <rdfs:range rdf:resource="http://www.w3.org/2001/XMLSchema#string"/>
  </owl:DatatypeProperty>
  <owl:DatatypeProperty rdf:about="http://example.org/onto/prop/google_storage_bucket_response_header">
    <rdfs:label>response_header</rdfs:label>
    <rdfs:comment>The list of HTTP headers other than the simple response headers to give permission for the user-agent to share across domains.</rdfs:comment>
    <rdfs:domain rdf:resource="http://example.org/onto/class/google_storage_bucket"/>
    <rdfs:range rdf:resource="http://www.w3.org/2001/XMLSchema#string"/>
  </owl:DatatypeProperty>
  <owl:DatatypeProperty rdf:about="http://example.org/onto/prop/google_storage_bucket_data_locations">
    <rdfs:label>data_locations</rdfs:label>
    <rdfs:comment>The list of individual regions that comprise a dual-region bucket. See the docs for a list of acceptable regions. Note: If any of the data_locations changes, it will recreate the bucket.</rdfs:comment>
    <rdfs:domain rdf:resource="http://example.org/onto/class/google_storage_bucket"/>
    <rdfs:range rdf:resource="http://www.w3.org/2001/XMLSchema#string"/>
  </owl:DatatypeProperty>
  <owl:DatatypeProperty rdf:about="http://example.org/onto/prop/google_storage_bucket_default_kms_key_name">
    <rdfs:label>default_kms_key_name</rdfs:label>
    <rdfs:comment>A Cloud KMS key that will be used to encrypt objects inserted into this bucket, if no encryption method is specified. You must pay attention to whether the crypto key is available in the location that this bucket is created in. See the docs for more details.</rdfs:comment>
    <rdfs:domain rdf:resource="http://example.org/onto/class/google_storage_bucket"/>
    <rdfs:range rdf:resource="http://www.w3.org/2001/XMLSchema#string"/>
  </owl:DatatypeProperty>
  <owl:DatatypeProperty rdf:about="http://example.org/onto/prop/google_storage_bucket_enabled">
    <rdfs:label>enabled</rdfs:label>
    <rdfs:comment>Set this field true to organize bucket with logical file system structure.</rdfs:comment>
    <rdfs:domain rdf:resource="http://example.org/onto/class/google_storage_bucket"/>
    <rdfs:range rdf:resource="http://www.w3.org/2001/XMLSchema#string"/>
  </owl:DatatypeProperty>
  <owl:DatatypeProperty rdf:about="http://example.org/onto/prop/google_storage_bucket_allow_all_service_agent_access">
    <rdfs:label>allow_all_service_agent_access</rdfs:label>
    <rdfs:comment>Whether to allow all service agents to access the bucket regardless of the IP filter configuration.</rdfs:comment>
    <rdfs:domain rdf:resource="http://example.org/onto/class/google_storage_bucket"/>
    <rdfs:range rdf:resource="http://www.w3.org/2001/XMLSchema#string"/>
  </owl:DatatypeProperty>
  <owl:DatatypeProperty rdf:about="http://example.org/onto/prop/google_storage_bucket_allow_cross_org_vpcs">
    <rdfs:label>allow_cross_org_vpcs</rdfs:label>
    <rdfs:comment>Whether to allow cross-org VPCs in the bucket's IP filter configuration.</rdfs:comment>
    <rdfs:domain rdf:resource="http://example.org/onto/class/google_storage_bucket"/>
    <rdfs:range rdf:resource="http://www.w3.org/2001/XMLSchema#string"/>
  </owl:DatatypeProperty>
  <owl:DatatypeProperty rdf:about="http://example.org/onto/prop/google_storage_bucket_mode">
    <rdfs:label>mode</rdfs:label>
    <rdfs:comment>The mode of the IP filter. Valid values are 'Enabled' and 'Disabled'.</rdfs:comment>
    <rdfs:domain rdf:resource="http://example.org/onto/class/google_storage_bucket"/>
    <rdfs:range rdf:resource="http://www.w3.org/2001/XMLSchema#string"/>
  </owl:DatatypeProperty>
  <owl:DatatypeProperty rdf:about="http://example.org/onto/prop/google_storage_bucket_allowed_ip_cidr_ranges">
    <rdfs:label>allowed_ip_cidr_ranges</rdfs:label>
    <rdfs:comment>The list of public IPv4, IPv6 cidr ranges that are allowed to access the bucket.</rdfs:comment>
    <rdfs:domain rdf:resource="http://example.org/onto/class/google_storage_bucket"/>
    <rdfs:range rdf:resource="http://www.w3.org/2001/XMLSchema#string"/>
  </owl:DatatypeProperty>
  <owl:DatatypeProperty rdf:about="http://example.org/onto/prop/google_storage_bucket_allowed_ip_cidr_ranges">
    <rdfs:label>allowed_ip_cidr_ranges</rdfs:label>
    <rdfs:comment>The list of public or private IPv4 and IPv6 CIDR ranges that can access the bucket.</rdfs:comment>
    <rdfs:domain rdf:resource="http://example.org/onto/class/google_storage_bucket"/>
    <rdfs:range rdf:resource="http://www.w3.org/2001/XMLSchema#string"/>
  </owl:DatatypeProperty>
  <owl:DatatypeProperty rdf:about="http://example.org/onto/prop/google_storage_bucket_network">
    <rdfs:label>network</rdfs:label>
    <rdfs:comment>Name of the network. Format: projects/{PROJECT_ID}/global/networks/{NETWORK_NAME}</rdfs:comment>
    <rdfs:domain rdf:resource="http://example.org/onto/class/google_storage_bucket"/>
    <rdfs:range rdf:resource="http://www.w3.org/2001/XMLSchema#string"/>
  </owl:DatatypeProperty>
  <owl:DatatypeProperty rdf:about="http://example.org/onto/prop/google_storage_bucket_storage_class">
    <rdfs:label>storage_class</rdfs:label>
    <rdfs:comment>The target Storage Class of objects affected by this Lifecycle Rule. Supported values include: MULTI_REGIONAL, REGIONAL, NEARLINE, COLDLINE, ARCHIVE.</rdfs:comment>
    <rdfs:domain rdf:resource="http://example.org/onto/class/google_storage_bucket"/>
    <rdfs:range rdf:resource="http://www.w3.org/2001/XMLSchema#string"/>
  </owl:DatatypeProperty>
  <owl:DatatypeProperty rdf:about="http://example.org/onto/prop/google_storage_bucket_type">
    <rdfs:label>type</rdfs:label>
    <rdfs:comment>The type of the action of this Lifecycle Rule. Supported values include: Delete, SetStorageClass and AbortIncompleteMultipartUpload.</rdfs:comment>
    <rdfs:domain rdf:resource="http://example.org/onto/class/google_storage_bucket"/>
    <rdfs:range rdf:resource="http://www.w3.org/2001/XMLSchema#string"/>
  </owl:DatatypeProperty>
  <owl:DatatypeProperty rdf:about="http://example.org/onto/prop/google_storage_bucket_age">
    <rdfs:label>age</rdfs:label>
    <rdfs:comment>Minimum age of an object in days to satisfy this condition.</rdfs:comment>
    <rdfs:domain rdf:resource="http://example.org/onto/class/google_storage_bucket"/>
    <rdfs:range rdf:resource="http://www.w3.org/2001/XMLSchema#string"/>
  </owl:DatatypeProperty>
  <owl:DatatypeProperty rdf:about="http://example.org/onto/prop/google_storage_bucket_created_before">
    <rdfs:label>created_before</rdfs:label>
    <rdfs:comment>Creation date of an object in RFC 3339 (e.g. 2017-06-13) to satisfy this condition.</rdfs:comment>
    <rdfs:domain rdf:resource="http://example.org/onto/class/google_storage_bucket"/>
    <rdfs:range rdf:resource="http://www.w3.org/2001/XMLSchema#string"/>
  </owl:DatatypeProperty>
  <owl:DatatypeProperty rdf:about="http://example.org/onto/prop/google_storage_bucket_custom_time_before">
    <rdfs:label>custom_time_before</rdfs:label>
    <rdfs:comment>Creation date of an object in RFC 3339 (e.g. 2017-06-13) to satisfy this condition.</rdfs:comment>
    <rdfs:domain rdf:resource="http://example.org/onto/class/google_storage_bucket"/>
    <rdfs:range rdf:resource="http://www.w3.org/2001/XMLSchema#string"/>
  </owl:DatatypeProperty>
  <owl:DatatypeProperty rdf:about="http://example.org/onto/prop/google_storage_bucket_days_since_custom_time">
    <rdfs:label>days_since_custom_time</rdfs:label>
    <rdfs:comment>Number of days elapsed since the user-specified timestamp set on an object.</rdfs:comment>
    <rdfs:domain rdf:resource="http://example.org/onto/class/google_storage_bucket"/>
    <rdfs:range rdf:resource="http://www.w3.org/2001/XMLSchema#string"/>
  </owl:DatatypeProperty>
  <owl:DatatypeProperty rdf:about="http://example.org/onto/prop/google_storage_bucket_days_since_noncurrent_time">
    <rdfs:label>days_since_noncurrent_time</rdfs:label>
    <rdfs:comment>Number of days elapsed since the noncurrent timestamp of an object. This
										condition is relevant only for versioned objects.</rdfs:comment>
    <rdfs:domain rdf:resource="http://example.org/onto/class/google_storage_bucket"/>
    <rdfs:range rdf:resource="http://www.w3.org/2001/XMLSchema#string"/>
  </owl:DatatypeProperty>
  <owl:DatatypeProperty rdf:about="http://example.org/onto/prop/google_storage_bucket_matches_prefix">
    <rdfs:label>matches_prefix</rdfs:label>
    <rdfs:comment>One or more matching name prefixes to satisfy this condition.</rdfs:comment>
    <rdfs:domain rdf:resource="http://example.org/onto/class/google_storage_bucket"/>
    <rdfs:range rdf:resource="http://www.w3.org/2001/XMLSchema#string"/>
  </owl:DatatypeProperty>
  <owl:DatatypeProperty rdf:about="http://example.org/onto/prop/google_storage_bucket_matches_storage_class">
    <rdfs:label>matches_storage_class</rdfs:label>
    <rdfs:comment>Storage Class of objects to satisfy this condition. Supported values include: MULTI_REGIONAL, REGIONAL, NEARLINE, COLDLINE, ARCHIVE, STANDARD, DURABLE_REDUCED_AVAILABILITY.</rdfs:comment>
    <rdfs:domain rdf:resource="http://example.org/onto/class/google_storage_bucket"/>
    <rdfs:range rdf:resource="http://www.w3.org/2001/XMLSchema#string"/>
  </owl:DatatypeProperty>
  <owl:DatatypeProperty rdf:about="http://example.org/onto/prop/google_storage_bucket_matches_suffix">
    <rdfs:label>matches_suffix</rdfs:label>
    <rdfs:comment>One or more matching name suffixes to satisfy this condition.</rdfs:comment>
    <rdfs:domain rdf:resource="http://example.org/onto/class/google_storage_bucket"/>
    <rdfs:range rdf:resource="http://www.w3.org/2001/XMLSchema#string"/>
  </owl:DatatypeProperty>
  <owl:DatatypeProperty rdf:about="http://example.org/onto/prop/google_storage_bucket_noncurrent_time_before">
    <rdfs:label>noncurrent_time_before</rdfs:label>
    <rdfs:comment>Creation date of an object in RFC 3339 (e.g. 2017-06-13) to satisfy this condition.</rdfs:comment>
    <rdfs:domain rdf:resource="http://example.org/onto/class/google_storage_bucket"/>
    <rdfs:range rdf:resource="http://www.w3.org/2001/XMLSchema#string"/>
  </owl:DatatypeProperty>
  <owl:DatatypeProperty rdf:about="http://example.org/onto/prop/google_storage_bucket_num_newer_versions">
    <rdfs:label>num_newer_versions</rdfs:label>
    <rdfs:comment>Relevant only for versioned objects. The number of newer versions of an object to satisfy this condition.</rdfs:comment>
    <rdfs:domain rdf:resource="http://example.org/onto/class/google_storage_bucket"/>
    <rdfs:range rdf:resource="http://www.w3.org/2001/XMLSchema#string"/>
  </owl:DatatypeProperty>
  <owl:DatatypeProperty rdf:about="http://example.org/onto/prop/google_storage_bucket_send_age_if_zero">
    <rdfs:label>send_age_if_zero</rdfs:label>
    <rdfs:comment>While set true, age value will be sent in the request even for zero value of the field. This field is only useful for setting 0 value to the age field. It can be used alone or together with age.</rdfs:comment>
    <rdfs:domain rdf:resource="http://example.org/onto/class/google_storage_bucket"/>
    <rdfs:range rdf:resource="http://www.w3.org/2001/XMLSchema#string"/>
  </owl:DatatypeProperty>
  <owl:DatatypeProperty rdf:about="http://example.org/onto/prop/google_storage_bucket_send_days_since_custom_time_if_zero">
    <rdfs:label>send_days_since_custom_time_if_zero</rdfs:label>
    <rdfs:comment>While set true, days_since_custom_time value will be sent in the request even for zero value of the field. This field is only useful for setting 0 value to the days_since_custom_time field. It can be used alone or together with days_since_custom_time.</rdfs:comment>
    <rdfs:domain rdf:resource="http://example.org/onto/class/google_storage_bucket"/>
    <rdfs:range rdf:resource="http://www.w3.org/2001/XMLSchema#string"/>
  </owl:DatatypeProperty>
  <owl:DatatypeProperty rdf:about="http://example.org/onto/prop/google_storage_bucket_send_days_since_noncurrent_time_if_zero">
    <rdfs:label>send_days_since_noncurrent_time_if_zero</rdfs:label>
    <rdfs:comment>While set true, days_since_noncurrent_time value will be sent in the request even for zero value of the field. This field is only useful for setting 0 value to the days_since_noncurrent_time field. It can be used alone or together with days_since_noncurrent_time.</rdfs:comment>
    <rdfs:domain rdf:resource="http://example.org/onto/class/google_storage_bucket"/>
    <rdfs:range rdf:resource="http://www.w3.org/2001/XMLSchema#string"/>
  </owl:DatatypeProperty>
  <owl:DatatypeProperty rdf:about="http://example.org/onto/prop/google_storage_bucket_send_num_newer_versions_if_zero">
    <rdfs:label>send_num_newer_versions_if_zero</rdfs:label>
    <rdfs:comment>While set true, num_newer_versions value will be sent in the request even for zero value of the field. This field is only useful for setting 0 value to the num_newer_versions field. It can be used alone or together with num_newer_versions.</rdfs:comment>
    <rdfs:domain rdf:resource="http://example.org/onto/class/google_storage_bucket"/>
    <rdfs:range rdf:resource="http://www.w3.org/2001/XMLSchema#string"/>
  </owl:DatatypeProperty>
  <owl:DatatypeProperty rdf:about="http://example.org/onto/prop/google_storage_bucket_with_state">
    <rdfs:label>with_state</rdfs:label>
    <rdfs:comment>Match to live and/or archived objects. Unversioned buckets have only live objects. Supported values include: "LIVE", "ARCHIVED", "ANY".</rdfs:comment>
    <rdfs:domain rdf:resource="http://example.org/onto/class/google_storage_bucket"/>
    <rdfs:range rdf:resource="http://www.w3.org/2001/XMLSchema#string"/>
  </owl:DatatypeProperty>
  <owl:DatatypeProperty rdf:about="http://example.org/onto/prop/google_storage_bucket_log_bucket">
    <rdfs:label>log_bucket</rdfs:label>
    <rdfs:comment>The bucket that will receive log objects.</rdfs:comment>
    <rdfs:domain rdf:resource="http://example.org/onto/class/google_storage_bucket"/>
    <rdfs:range rdf:resource="http://www.w3.org/2001/XMLSchema#string"/>
  </owl:DatatypeProperty>
  <owl:DatatypeProperty rdf:about="http://example.org/onto/prop/google_storage_bucket_log_object_prefix">
    <rdfs:label>log_object_prefix</rdfs:label>
    <rdfs:comment>The object prefix for log objects. If it's not provided, by default Google Cloud Storage sets this to this bucket's name.</rdfs:comment>
    <rdfs:domain rdf:resource="http://example.org/onto/class/google_storage_bucket"/>
    <rdfs:range rdf:resource="http://www.w3.org/2001/XMLSchema#string"/>
  </owl:DatatypeProperty>
  <owl:DatatypeProperty rdf:about="http://example.org/onto/prop/google_storage_bucket_is_locked">
    <rdfs:label>is_locked</rdfs:label>
    <rdfs:comment>If set to true, the bucket will be locked and permanently restrict edits to the bucket's retention policy.  Caution: Locking a bucket is an irreversible action.</rdfs:comment>
    <rdfs:domain rdf:resource="http://example.org/onto/class/google_storage_bucket"/>
    <rdfs:range rdf:resource="http://www.w3.org/2001/XMLSchema#string"/>
  </owl:DatatypeProperty>
  <owl:DatatypeProperty rdf:about="http://example.org/onto/prop/google_storage_bucket_retention_period">
    <rdfs:label>retention_period</rdfs:label>
    <rdfs:comment>The period of time, in seconds, that objects in the bucket must be retained and cannot be deleted, overwritten, or archived. The value must be less than 3,155,760,000 seconds.</rdfs:comment>
    <rdfs:domain rdf:resource="http://example.org/onto/class/google_storage_bucket"/>
    <rdfs:range rdf:resource="http://www.w3.org/2001/XMLSchema#string"/>
  </owl:DatatypeProperty>
  <owl:DatatypeProperty rdf:about="http://example.org/onto/prop/google_storage_bucket_effective_time">
    <rdfs:label>effective_time</rdfs:label>
    <rdfs:comment>Server-determined value that indicates the time from which the policy, or one with a greater retention, was effective. This value is in RFC 3339 format.</rdfs:comment>
    <rdfs:domain rdf:resource="http://example.org/onto/class/google_storage_bucket"/>
    <rdfs:range rdf:resource="http://www.w3.org/2001/XMLSchema#string"/>
  </owl:DatatypeProperty>
  <owl:DatatypeProperty rdf:about="http://example.org/onto/prop/google_storage_bucket_retention_duration_seconds">
    <rdfs:label>retention_duration_seconds</rdfs:label>
    <rdfs:comment>The duration in seconds that soft-deleted objects in the bucket will be retained and cannot be permanently deleted. Default value is 604800.</rdfs:comment>
    <rdfs:domain rdf:resource="http://example.org/onto/class/google_storage_bucket"/>
    <rdfs:range rdf:resource="http://www.w3.org/2001/XMLSchema#string"/>
  </owl:DatatypeProperty>
  <owl:DatatypeProperty rdf:about="http://example.org/onto/prop/google_storage_bucket_create">
    <rdfs:label>create</rdfs:label>
    <rdfs:domain rdf:resource="http://example.org/onto/class/google_storage_bucket"/>
    <rdfs:range rdf:resource="http://www.w3.org/2001/XMLSchema#string"/>
  </owl:DatatypeProperty>
  <owl:DatatypeProperty rdf:about="http://example.org/onto/prop/google_storage_bucket_read">
    <rdfs:label>read</rdfs:label>
    <rdfs:domain rdf:resource="http://example.org/onto/class/google_storage_bucket"/>
    <rdfs:range rdf:resource="http://www.w3.org/2001/XMLSchema#string"/>
  </owl:DatatypeProperty>
  <owl:DatatypeProperty rdf:about="http://example.org/onto/prop/google_storage_bucket_update">
    <rdfs:label>update</rdfs:label>
    <rdfs:domain rdf:resource="http://example.org/onto/class/google_storage_bucket"/>
    <rdfs:range rdf:resource="http://www.w3.org/2001/XMLSchema#string"/>
  </owl:DatatypeProperty>
  <owl:DatatypeProperty rdf:about="http://example.org/onto/prop/google_storage_bucket_enabled">
    <rdfs:label>enabled</rdfs:label>
    <rdfs:comment>While set to true, versioning is fully enabled for this bucket.</rdfs:comment>
    <rdfs:domain rdf:resource="http://example.org/onto/class/google_storage_bucket"/>
    <rdfs:range rdf:resource="http://www.w3.org/2001/XMLSchema#string"/>
  </owl:DatatypeProperty>
  <owl:DatatypeProperty rdf:about="http://example.org/onto/prop/google_storage_bucket_main_page_suffix">
    <rdfs:label>main_page_suffix</rdfs:label>
    <rdfs:comment>Behaves as the bucket's directory index where missing objects are treated as potential directories.</rdfs:comment>
    <rdfs:domain rdf:resource="http://example.org/onto/class/google_storage_bucket"/>
    <rdfs:range rdf:resource="http://www.w3.org/2001/XMLSchema#string"/>
  </owl:DatatypeProperty>
  <owl:DatatypeProperty rdf:about="http://example.org/onto/prop/google_storage_bucket_not_found_page">
    <rdfs:label>not_found_page</rdfs:label>
    <rdfs:comment>The custom object to return when a requested resource is not found.</rdfs:comment>
    <rdfs:domain rdf:resource="http://example.org/onto/class/google_storage_bucket"/>
    <rdfs:range rdf:resource="http://www.w3.org/2001/XMLSchema#string"/>
  </owl:DatatypeProperty>
</rdf:RDF>
