<?xml version="1.0" encoding="UTF-8"?>
<rdf:RDF
  xmlns:rdf="http://www.w3.org/1999/02/22-rdf-syntax-ns#"
  xmlns:rdfs="http://www.w3.org/2000/01/rdf-schema#"
  xmlns:owl="http://www.w3.org/2002/07/owl#"
  xmlns:xsd="http://www.w3.org/2001/XMLSchema#"
  xml:base="http://example.org/onto/">
  <owl:Class rdf:about="http://example.org/onto/class/google_sql_source_representation_instance">
    <rdfs:label>google_sql_source_representation_instance</rdfs:label>
    <rdfs:comment>#
#     ***     AUTO GENERATED CODE    ***    Type: MMv1     ***
#
# ----------------------------------------------------------------------------
#
#     This code is generated by Magic Modules using the following:
#
#     Configuration: https:#github.com/GoogleCloudPlatform/magic-modules/tree/main/mmv1/products/sql/SourceRepresentationInstance.yaml
#     Template:      https:#github.com/GoogleCloudPlatform/magic-modules/tree/main/mmv1/templates/terraform/resource.html.markdown.tmpl
#
#     DO NOT EDIT this file directly. Any changes made to this file will be
#     overwritten during the next generation cycle.
#
# ----------------------------------------------------------------------------
subcategory: "Cloud SQL"
description: |-
  A source representation instance is a Cloud SQL instance that represents
  the source database server to the Cloud SQL replica.
---</rdfs:comment>
  </owl:Class>
  <owl:DatatypeProperty rdf:about="http://example.org/onto/prop/google_sql_source_representation_instance_ca_certificate">
    <rdfs:label>ca_certificate</rdfs:label>
    <rdfs:comment>The CA certificate on the external server. Include only if SSL/TLS is used on the external server.</rdfs:comment>
    <rdfs:domain rdf:resource="http://example.org/onto/class/google_sql_source_representation_instance"/>
    <rdfs:range rdf:resource="http://www.w3.org/2001/XMLSchema#string"/>
  </owl:DatatypeProperty>
  <owl:DatatypeProperty rdf:about="http://example.org/onto/prop/google_sql_source_representation_instance_client_certificate">
    <rdfs:label>client_certificate</rdfs:label>
    <rdfs:comment>The client certificate on the external server. Required only for server-client authentication. Include only if SSL/TLS is used on the external server.</rdfs:comment>
    <rdfs:domain rdf:resource="http://example.org/onto/class/google_sql_source_representation_instance"/>
    <rdfs:range rdf:resource="http://www.w3.org/2001/XMLSchema#string"/>
  </owl:DatatypeProperty>
  <owl:DatatypeProperty rdf:about="http://example.org/onto/prop/google_sql_source_representation_instance_client_key">
    <rdfs:label>client_key</rdfs:label>
    <rdfs:comment>The private key file for the client certificate on the external server. Required only for server-client authentication. Include only if SSL/TLS is used on the external server.</rdfs:comment>
    <rdfs:domain rdf:resource="http://example.org/onto/class/google_sql_source_representation_instance"/>
    <rdfs:range rdf:resource="http://www.w3.org/2001/XMLSchema#string"/>
  </owl:DatatypeProperty>
  <owl:DatatypeProperty rdf:about="http://example.org/onto/prop/google_sql_source_representation_instance_database_version">
    <rdfs:label>database_version</rdfs:label>
    <rdfs:comment>The MySQL, PostgreSQL or SQL Server (beta) version to use. Supported values include MYSQL_5_6, MYSQL_5_7, MYSQL_8_0, MYSQL_8_4, POSTGRES_9_6, POSTGRES_10, POSTGRES_11, POSTGRES_12, POSTGRES_13, POSTGRES_14, POSTGRES_15, POSTGRES_16, POSTGRES_17. Database Version Policies includes an up-to-date reference of supported versions.</rdfs:comment>
    <rdfs:domain rdf:resource="http://example.org/onto/class/google_sql_source_representation_instance"/>
    <rdfs:range rdf:resource="http://www.w3.org/2001/XMLSchema#string"/>
  </owl:DatatypeProperty>
  <owl:DatatypeProperty rdf:about="http://example.org/onto/prop/google_sql_source_representation_instance_dump_file_path">
    <rdfs:label>dump_file_path</rdfs:label>
    <rdfs:comment>A file in the bucket that contains the data from the external server.</rdfs:comment>
    <rdfs:domain rdf:resource="http://example.org/onto/class/google_sql_source_representation_instance"/>
    <rdfs:range rdf:resource="http://www.w3.org/2001/XMLSchema#string"/>
  </owl:DatatypeProperty>
  <owl:DatatypeProperty rdf:about="http://example.org/onto/prop/google_sql_source_representation_instance_host">
    <rdfs:label>host</rdfs:label>
    <rdfs:comment>The IPv4 address and port for the external server, or the the DNS address for the external server. If the external server is hosted on Cloud SQL, the port is 5432.</rdfs:comment>
    <rdfs:domain rdf:resource="http://example.org/onto/class/google_sql_source_representation_instance"/>
    <rdfs:range rdf:resource="http://www.w3.org/2001/XMLSchema#string"/>
  </owl:DatatypeProperty>
  <owl:DatatypeProperty rdf:about="http://example.org/onto/prop/google_sql_source_representation_instance_id">
    <rdfs:label>id</rdfs:label>
    <rdfs:domain rdf:resource="http://example.org/onto/class/google_sql_source_representation_instance"/>
    <rdfs:range rdf:resource="http://www.w3.org/2001/XMLSchema#string"/>
  </owl:DatatypeProperty>
  <owl:DatatypeProperty rdf:about="http://example.org/onto/prop/google_sql_source_representation_instance_name">
    <rdfs:label>name</rdfs:label>
    <rdfs:comment>The name of the source representation instance. Use any valid Cloud SQL instance name.</rdfs:comment>
    <rdfs:domain rdf:resource="http://example.org/onto/class/google_sql_source_representation_instance"/>
    <rdfs:range rdf:resource="http://www.w3.org/2001/XMLSchema#string"/>
  </owl:DatatypeProperty>
  <owl:DatatypeProperty rdf:about="http://example.org/onto/prop/google_sql_source_representation_instance_password">
    <rdfs:label>password</rdfs:label>
    <rdfs:comment>The password for the replication user account.</rdfs:comment>
    <rdfs:domain rdf:resource="http://example.org/onto/class/google_sql_source_representation_instance"/>
    <rdfs:range rdf:resource="http://www.w3.org/2001/XMLSchema#string"/>
  </owl:DatatypeProperty>
  <owl:DatatypeProperty rdf:about="http://example.org/onto/prop/google_sql_source_representation_instance_port">
    <rdfs:label>port</rdfs:label>
    <rdfs:comment>The externally accessible port for the source database server.
Defaults to 3306.</rdfs:comment>
    <rdfs:domain rdf:resource="http://example.org/onto/class/google_sql_source_representation_instance"/>
    <rdfs:range rdf:resource="http://www.w3.org/2001/XMLSchema#string"/>
  </owl:DatatypeProperty>
  <owl:DatatypeProperty rdf:about="http://example.org/onto/prop/google_sql_source_representation_instance_project">
    <rdfs:label>project</rdfs:label>
    <rdfs:domain rdf:resource="http://example.org/onto/class/google_sql_source_representation_instance"/>
    <rdfs:range rdf:resource="http://www.w3.org/2001/XMLSchema#string"/>
  </owl:DatatypeProperty>
  <owl:DatatypeProperty rdf:about="http://example.org/onto/prop/google_sql_source_representation_instance_region">
    <rdfs:label>region</rdfs:label>
    <rdfs:comment>The Region in which the created instance should reside.
If it is not provided, the provider region is used.</rdfs:comment>
    <rdfs:domain rdf:resource="http://example.org/onto/class/google_sql_source_representation_instance"/>
    <rdfs:range rdf:resource="http://www.w3.org/2001/XMLSchema#string"/>
  </owl:DatatypeProperty>
  <owl:DatatypeProperty rdf:about="http://example.org/onto/prop/google_sql_source_representation_instance_username">
    <rdfs:label>username</rdfs:label>
    <rdfs:comment>The replication user account on the external server.</rdfs:comment>
    <rdfs:domain rdf:resource="http://example.org/onto/class/google_sql_source_representation_instance"/>
    <rdfs:range rdf:resource="http://www.w3.org/2001/XMLSchema#string"/>
  </owl:DatatypeProperty>
  <owl:DatatypeProperty rdf:about="http://example.org/onto/prop/google_sql_source_representation_instance_create">
    <rdfs:label>create</rdfs:label>
    <rdfs:domain rdf:resource="http://example.org/onto/class/google_sql_source_representation_instance"/>
    <rdfs:range rdf:resource="http://www.w3.org/2001/XMLSchema#string"/>
  </owl:DatatypeProperty>
  <owl:DatatypeProperty rdf:about="http://example.org/onto/prop/google_sql_source_representation_instance_delete">
    <rdfs:label>delete</rdfs:label>
    <rdfs:domain rdf:resource="http://example.org/onto/class/google_sql_source_representation_instance"/>
    <rdfs:range rdf:resource="http://www.w3.org/2001/XMLSchema#string"/>
  </owl:DatatypeProperty>
</rdf:RDF>
