<?xml version="1.0" encoding="UTF-8"?>
<rdf:RDF
  xmlns:rdf="http://www.w3.org/1999/02/22-rdf-syntax-ns#"
  xmlns:rdfs="http://www.w3.org/2000/01/rdf-schema#"
  xmlns:owl="http://www.w3.org/2002/07/owl#"
  xmlns:xsd="http://www.w3.org/2001/XMLSchema#"
  xml:base="http://example.org/onto/">
  <owl:Class rdf:about="http://example.org/onto/class/google_org_policy_custom_constraint">
    <rdfs:label>google_org_policy_custom_constraint</rdfs:label>
    <rdfs:comment>#
#     ***     AUTO GENERATED CODE    ***    Type: MMv1     ***
#
# ----------------------------------------------------------------------------
#
#     This code is generated by Magic Modules using the following:
#
#     Configuration: https:#github.com/GoogleCloudPlatform/magic-modules/tree/main/mmv1/products/orgpolicy/CustomConstraint.yaml
#     Template:      https:#github.com/GoogleCloudPlatform/magic-modules/tree/main/mmv1/templates/terraform/resource.html.markdown.tmpl
#
#     DO NOT EDIT this file directly. Any changes made to this file will be
#     overwritten during the next generation cycle.
#
# ----------------------------------------------------------------------------
subcategory: "Organization Policy"
description: |-
  Custom constraints are created by administrators to provide more granular and customizable control over the specific fields that are restricted by your organization policies.
---</rdfs:comment>
  </owl:Class>
  <owl:DatatypeProperty rdf:about="http://example.org/onto/prop/google_org_policy_custom_constraint_action_type">
    <rdfs:label>action_type</rdfs:label>
    <rdfs:comment>The action to take if the condition is met. Possible values: ["ALLOW", "DENY"]</rdfs:comment>
    <rdfs:domain rdf:resource="http://example.org/onto/class/google_org_policy_custom_constraint"/>
    <rdfs:range rdf:resource="http://www.w3.org/2001/XMLSchema#string"/>
  </owl:DatatypeProperty>
  <owl:DatatypeProperty rdf:about="http://example.org/onto/prop/google_org_policy_custom_constraint_condition">
    <rdfs:label>condition</rdfs:label>
    <rdfs:comment>A CEL condition that refers to a supported service resource, for example 'resource.management.autoUpgrade == false'. For details about CEL usage, see [Common Expression Language](https://cloud.google.com/resource-manager/docs/organization-policy/creating-managing-custom-constraints#common_expression_language).</rdfs:comment>
    <rdfs:domain rdf:resource="http://example.org/onto/class/google_org_policy_custom_constraint"/>
    <rdfs:range rdf:resource="http://www.w3.org/2001/XMLSchema#string"/>
  </owl:DatatypeProperty>
  <owl:DatatypeProperty rdf:about="http://example.org/onto/prop/google_org_policy_custom_constraint_description">
    <rdfs:label>description</rdfs:label>
    <rdfs:comment>A human-friendly description of the constraint to display as an error message when the policy is violated.</rdfs:comment>
    <rdfs:domain rdf:resource="http://example.org/onto/class/google_org_policy_custom_constraint"/>
    <rdfs:range rdf:resource="http://www.w3.org/2001/XMLSchema#string"/>
  </owl:DatatypeProperty>
  <owl:DatatypeProperty rdf:about="http://example.org/onto/prop/google_org_policy_custom_constraint_display_name">
    <rdfs:label>display_name</rdfs:label>
    <rdfs:comment>A human-friendly name for the constraint.</rdfs:comment>
    <rdfs:domain rdf:resource="http://example.org/onto/class/google_org_policy_custom_constraint"/>
    <rdfs:range rdf:resource="http://www.w3.org/2001/XMLSchema#string"/>
  </owl:DatatypeProperty>
  <owl:DatatypeProperty rdf:about="http://example.org/onto/prop/google_org_policy_custom_constraint_id">
    <rdfs:label>id</rdfs:label>
    <rdfs:domain rdf:resource="http://example.org/onto/class/google_org_policy_custom_constraint"/>
    <rdfs:range rdf:resource="http://www.w3.org/2001/XMLSchema#string"/>
  </owl:DatatypeProperty>
  <owl:DatatypeProperty rdf:about="http://example.org/onto/prop/google_org_policy_custom_constraint_method_types">
    <rdfs:label>method_types</rdfs:label>
    <rdfs:comment>A list of RESTful methods for which to enforce the constraint. Can be 'CREATE', 'UPDATE', or both. Not all Google Cloud services support both methods. To see supported methods for each service, find the service in [Supported services](https://cloud.google.com/resource-manager/docs/organization-policy/custom-constraint-supported-services).</rdfs:comment>
    <rdfs:domain rdf:resource="http://example.org/onto/class/google_org_policy_custom_constraint"/>
    <rdfs:range rdf:resource="http://www.w3.org/2001/XMLSchema#string"/>
  </owl:DatatypeProperty>
  <owl:DatatypeProperty rdf:about="http://example.org/onto/prop/google_org_policy_custom_constraint_name">
    <rdfs:label>name</rdfs:label>
    <rdfs:comment>Immutable. The name of the custom constraint. This is unique within the organization.</rdfs:comment>
    <rdfs:domain rdf:resource="http://example.org/onto/class/google_org_policy_custom_constraint"/>
    <rdfs:range rdf:resource="http://www.w3.org/2001/XMLSchema#string"/>
  </owl:DatatypeProperty>
  <owl:DatatypeProperty rdf:about="http://example.org/onto/prop/google_org_policy_custom_constraint_parent">
    <rdfs:label>parent</rdfs:label>
    <rdfs:comment>The parent of the resource, an organization. Format should be 'organizations/{organization_id}'.</rdfs:comment>
    <rdfs:domain rdf:resource="http://example.org/onto/class/google_org_policy_custom_constraint"/>
    <rdfs:range rdf:resource="http://www.w3.org/2001/XMLSchema#string"/>
  </owl:DatatypeProperty>
  <owl:DatatypeProperty rdf:about="http://example.org/onto/prop/google_org_policy_custom_constraint_resource_types">
    <rdfs:label>resource_types</rdfs:label>
    <rdfs:comment>Immutable. The fully qualified name of the Google Cloud REST resource containing the object and field you want to restrict. For example, 'container.googleapis.com/NodePool'.</rdfs:comment>
    <rdfs:domain rdf:resource="http://example.org/onto/class/google_org_policy_custom_constraint"/>
    <rdfs:range rdf:resource="http://www.w3.org/2001/XMLSchema#string"/>
  </owl:DatatypeProperty>
  <owl:DatatypeProperty rdf:about="http://example.org/onto/prop/google_org_policy_custom_constraint_update_time">
    <rdfs:label>update_time</rdfs:label>
    <rdfs:comment>Output only. The timestamp representing when the constraint was last updated.</rdfs:comment>
    <rdfs:domain rdf:resource="http://example.org/onto/class/google_org_policy_custom_constraint"/>
    <rdfs:range rdf:resource="http://www.w3.org/2001/XMLSchema#string"/>
  </owl:DatatypeProperty>
  <owl:DatatypeProperty rdf:about="http://example.org/onto/prop/google_org_policy_custom_constraint_create">
    <rdfs:label>create</rdfs:label>
    <rdfs:domain rdf:resource="http://example.org/onto/class/google_org_policy_custom_constraint"/>
    <rdfs:range rdf:resource="http://www.w3.org/2001/XMLSchema#string"/>
  </owl:DatatypeProperty>
  <owl:DatatypeProperty rdf:about="http://example.org/onto/prop/google_org_policy_custom_constraint_delete">
    <rdfs:label>delete</rdfs:label>
    <rdfs:domain rdf:resource="http://example.org/onto/class/google_org_policy_custom_constraint"/>
    <rdfs:range rdf:resource="http://www.w3.org/2001/XMLSchema#string"/>
  </owl:DatatypeProperty>
  <owl:DatatypeProperty rdf:about="http://example.org/onto/prop/google_org_policy_custom_constraint_update">
    <rdfs:label>update</rdfs:label>
    <rdfs:domain rdf:resource="http://example.org/onto/class/google_org_policy_custom_constraint"/>
    <rdfs:range rdf:resource="http://www.w3.org/2001/XMLSchema#string"/>
  </owl:DatatypeProperty>
</rdf:RDF>
