<?xml version="1.0" encoding="UTF-8"?>
<rdf:RDF
  xmlns:rdf="http://www.w3.org/1999/02/22-rdf-syntax-ns#"
  xmlns:rdfs="http://www.w3.org/2000/01/rdf-schema#"
  xmlns:owl="http://www.w3.org/2002/07/owl#"
  xmlns:xsd="http://www.w3.org/2001/XMLSchema#"
  xml:base="http://example.org/onto/">
  <owl:Class rdf:about="http://example.org/onto/class/google_monitoring_notification_channel">
    <rdfs:label>google_monitoring_notification_channel</rdfs:label>
    <rdfs:comment>#
#     ***     AUTO GENERATED CODE    ***    Type: MMv1     ***
#
# ----------------------------------------------------------------------------
#
#     This code is generated by Magic Modules using the following:
#
#     Configuration: https:#github.com/GoogleCloudPlatform/magic-modules/tree/main/mmv1/products/monitoring/NotificationChannel.yaml
#     Template:      https:#github.com/GoogleCloudPlatform/magic-modules/tree/main/mmv1/templates/terraform/resource.html.markdown.tmpl
#
#     DO NOT EDIT this file directly. Any changes made to this file will be
#     overwritten during the next generation cycle.
#
# ----------------------------------------------------------------------------
subcategory: "Cloud (Stackdriver) Monitoring"
description: |-
  A NotificationChannel is a medium through which an alert is delivered
  when a policy violation is detected.
---</rdfs:comment>
  </owl:Class>
  <owl:DatatypeProperty rdf:about="http://example.org/onto/prop/google_monitoring_notification_channel_description">
    <rdfs:label>description</rdfs:label>
    <rdfs:comment>An optional human-readable description of this notification channel. This description may provide additional details, beyond the display name, for the channel. This may not exceed 1024 Unicode characters.</rdfs:comment>
    <rdfs:domain rdf:resource="http://example.org/onto/class/google_monitoring_notification_channel"/>
    <rdfs:range rdf:resource="http://www.w3.org/2001/XMLSchema#string"/>
  </owl:DatatypeProperty>
  <owl:DatatypeProperty rdf:about="http://example.org/onto/prop/google_monitoring_notification_channel_display_name">
    <rdfs:label>display_name</rdfs:label>
    <rdfs:comment>An optional human-readable name for this notification channel. It is recommended that you specify a non-empty and unique name in order to make it easier to identify the channels in your project, though this is not enforced. The display name is limited to 512 Unicode characters.</rdfs:comment>
    <rdfs:domain rdf:resource="http://example.org/onto/class/google_monitoring_notification_channel"/>
    <rdfs:range rdf:resource="http://www.w3.org/2001/XMLSchema#string"/>
  </owl:DatatypeProperty>
  <owl:DatatypeProperty rdf:about="http://example.org/onto/prop/google_monitoring_notification_channel_enabled">
    <rdfs:label>enabled</rdfs:label>
    <rdfs:comment>Whether notifications are forwarded to the described channel. This makes it possible to disable delivery of notifications to a particular channel without removing the channel from all alerting policies that reference the channel. This is a more convenient approach when the change is temporary and you want to receive notifications from the same set of alerting policies on the channel at some point in the future.</rdfs:comment>
    <rdfs:domain rdf:resource="http://example.org/onto/class/google_monitoring_notification_channel"/>
    <rdfs:range rdf:resource="http://www.w3.org/2001/XMLSchema#string"/>
  </owl:DatatypeProperty>
  <owl:DatatypeProperty rdf:about="http://example.org/onto/prop/google_monitoring_notification_channel_force_delete">
    <rdfs:label>force_delete</rdfs:label>
    <rdfs:comment>If true, the notification channel will be deleted regardless
of its use in alert policies (the policies will be updated
to remove the channel). If false, channels that are still
referenced by an existing alerting policy will fail to be
deleted in a delete operation.</rdfs:comment>
    <rdfs:domain rdf:resource="http://example.org/onto/class/google_monitoring_notification_channel"/>
    <rdfs:range rdf:resource="http://www.w3.org/2001/XMLSchema#string"/>
  </owl:DatatypeProperty>
  <owl:DatatypeProperty rdf:about="http://example.org/onto/prop/google_monitoring_notification_channel_id">
    <rdfs:label>id</rdfs:label>
    <rdfs:domain rdf:resource="http://example.org/onto/class/google_monitoring_notification_channel"/>
    <rdfs:range rdf:resource="http://www.w3.org/2001/XMLSchema#string"/>
  </owl:DatatypeProperty>
  <owl:DatatypeProperty rdf:about="http://example.org/onto/prop/google_monitoring_notification_channel_labels">
    <rdfs:label>labels</rdfs:label>
    <rdfs:comment>Configuration fields that define the channel and its behavior. The
permissible and required labels are specified in the
NotificationChannelDescriptor corresponding to the type field.

Labels with sensitive data are obfuscated by the API and therefore Terraform cannot
determine if there are upstream changes to these fields. They can also be configured via
the sensitive_labels block, but cannot be configured in both places.</rdfs:comment>
    <rdfs:domain rdf:resource="http://example.org/onto/class/google_monitoring_notification_channel"/>
    <rdfs:range rdf:resource="http://www.w3.org/2001/XMLSchema#string"/>
  </owl:DatatypeProperty>
  <owl:DatatypeProperty rdf:about="http://example.org/onto/prop/google_monitoring_notification_channel_name">
    <rdfs:label>name</rdfs:label>
    <rdfs:comment>The full REST resource name for this channel. The syntax is:
projects/[PROJECT_ID]/notificationChannels/[CHANNEL_ID]
The [CHANNEL_ID] is automatically assigned by the server on creation.</rdfs:comment>
    <rdfs:domain rdf:resource="http://example.org/onto/class/google_monitoring_notification_channel"/>
    <rdfs:range rdf:resource="http://www.w3.org/2001/XMLSchema#string"/>
  </owl:DatatypeProperty>
  <owl:DatatypeProperty rdf:about="http://example.org/onto/prop/google_monitoring_notification_channel_project">
    <rdfs:label>project</rdfs:label>
    <rdfs:domain rdf:resource="http://example.org/onto/class/google_monitoring_notification_channel"/>
    <rdfs:range rdf:resource="http://www.w3.org/2001/XMLSchema#string"/>
  </owl:DatatypeProperty>
  <owl:DatatypeProperty rdf:about="http://example.org/onto/prop/google_monitoring_notification_channel_type">
    <rdfs:label>type</rdfs:label>
    <rdfs:comment>The type of the notification channel. This field matches the value of the NotificationChannelDescriptor.type field. See https://cloud.google.com/monitoring/api/ref_v3/rest/v3/projects.notificationChannelDescriptors/list to get the list of valid values such as "email", "slack", etc...</rdfs:comment>
    <rdfs:domain rdf:resource="http://example.org/onto/class/google_monitoring_notification_channel"/>
    <rdfs:range rdf:resource="http://www.w3.org/2001/XMLSchema#string"/>
  </owl:DatatypeProperty>
  <owl:DatatypeProperty rdf:about="http://example.org/onto/prop/google_monitoring_notification_channel_user_labels">
    <rdfs:label>user_labels</rdfs:label>
    <rdfs:comment>User-supplied key/value data that does not need to conform to the corresponding NotificationChannelDescriptor's schema, unlike the labels field. This field is intended to be used for organizing and identifying the NotificationChannel objects.The field can contain up to 64 entries. Each key and value is limited to 63 Unicode characters or 128 bytes, whichever is smaller. Labels and values can contain only lowercase letters, numerals, underscores, and dashes. Keys must begin with a letter.</rdfs:comment>
    <rdfs:domain rdf:resource="http://example.org/onto/class/google_monitoring_notification_channel"/>
    <rdfs:range rdf:resource="http://www.w3.org/2001/XMLSchema#string"/>
  </owl:DatatypeProperty>
  <owl:DatatypeProperty rdf:about="http://example.org/onto/prop/google_monitoring_notification_channel_verification_status">
    <rdfs:label>verification_status</rdfs:label>
    <rdfs:comment>Indicates whether this channel has been verified or not. On a ListNotificationChannels or GetNotificationChannel operation, this field is expected to be populated.If the value is UNVERIFIED, then it indicates that the channel is non-functioning (it both requires verification and lacks verification); otherwise, it is assumed that the channel works.If the channel is neither VERIFIED nor UNVERIFIED, it implies that the channel is of a type that does not require verification or that this specific channel has been exempted from verification because it was created prior to verification being required for channels of this type.This field cannot be modified using a standard UpdateNotificationChannel operation. To change the value of this field, you must call VerifyNotificationChannel.</rdfs:comment>
    <rdfs:domain rdf:resource="http://example.org/onto/class/google_monitoring_notification_channel"/>
    <rdfs:range rdf:resource="http://www.w3.org/2001/XMLSchema#string"/>
  </owl:DatatypeProperty>
  <owl:DatatypeProperty rdf:about="http://example.org/onto/prop/google_monitoring_notification_channel_auth_token">
    <rdfs:label>auth_token</rdfs:label>
    <rdfs:comment>An authorization token for a notification channel. Channel types that support this field include: slack</rdfs:comment>
    <rdfs:domain rdf:resource="http://example.org/onto/class/google_monitoring_notification_channel"/>
    <rdfs:range rdf:resource="http://www.w3.org/2001/XMLSchema#string"/>
  </owl:DatatypeProperty>
  <owl:DatatypeProperty rdf:about="http://example.org/onto/prop/google_monitoring_notification_channel_password">
    <rdfs:label>password</rdfs:label>
    <rdfs:comment>An password for a notification channel. Channel types that support this field include: webhook_basicauth</rdfs:comment>
    <rdfs:domain rdf:resource="http://example.org/onto/class/google_monitoring_notification_channel"/>
    <rdfs:range rdf:resource="http://www.w3.org/2001/XMLSchema#string"/>
  </owl:DatatypeProperty>
  <owl:DatatypeProperty rdf:about="http://example.org/onto/prop/google_monitoring_notification_channel_service_key">
    <rdfs:label>service_key</rdfs:label>
    <rdfs:comment>An servicekey token for a notification channel. Channel types that support this field include: pagerduty</rdfs:comment>
    <rdfs:domain rdf:resource="http://example.org/onto/class/google_monitoring_notification_channel"/>
    <rdfs:range rdf:resource="http://www.w3.org/2001/XMLSchema#string"/>
  </owl:DatatypeProperty>
  <owl:DatatypeProperty rdf:about="http://example.org/onto/prop/google_monitoring_notification_channel_create">
    <rdfs:label>create</rdfs:label>
    <rdfs:domain rdf:resource="http://example.org/onto/class/google_monitoring_notification_channel"/>
    <rdfs:range rdf:resource="http://www.w3.org/2001/XMLSchema#string"/>
  </owl:DatatypeProperty>
  <owl:DatatypeProperty rdf:about="http://example.org/onto/prop/google_monitoring_notification_channel_delete">
    <rdfs:label>delete</rdfs:label>
    <rdfs:domain rdf:resource="http://example.org/onto/class/google_monitoring_notification_channel"/>
    <rdfs:range rdf:resource="http://www.w3.org/2001/XMLSchema#string"/>
  </owl:DatatypeProperty>
  <owl:DatatypeProperty rdf:about="http://example.org/onto/prop/google_monitoring_notification_channel_update">
    <rdfs:label>update</rdfs:label>
    <rdfs:domain rdf:resource="http://example.org/onto/class/google_monitoring_notification_channel"/>
    <rdfs:range rdf:resource="http://www.w3.org/2001/XMLSchema#string"/>
  </owl:DatatypeProperty>
</rdf:RDF>
