<?xml version="1.0" encoding="UTF-8"?>
<rdf:RDF
  xmlns:rdf="http://www.w3.org/1999/02/22-rdf-syntax-ns#"
  xmlns:rdfs="http://www.w3.org/2000/01/rdf-schema#"
  xmlns:owl="http://www.w3.org/2002/07/owl#"
  xmlns:xsd="http://www.w3.org/2001/XMLSchema#"
  xml:base="http://example.org/onto/">
  <owl:Class rdf:about="http://example.org/onto/class/google_filestore_backup">
    <rdfs:label>google_filestore_backup</rdfs:label>
    <rdfs:comment>#
#     ***     AUTO GENERATED CODE    ***    Type: MMv1     ***
#
# ----------------------------------------------------------------------------
#
#     This code is generated by Magic Modules using the following:
#
#     Configuration: https:#github.com/GoogleCloudPlatform/magic-modules/tree/main/mmv1/products/filestore/Backup.yaml
#     Template:      https:#github.com/GoogleCloudPlatform/magic-modules/tree/main/mmv1/templates/terraform/resource.html.markdown.tmpl
#
#     DO NOT EDIT this file directly. Any changes made to this file will be
#     overwritten during the next generation cycle.
#
# ----------------------------------------------------------------------------
subcategory: "Filestore"
description: |-
  A Google Cloud Filestore backup.
---</rdfs:comment>
  </owl:Class>
  <owl:DatatypeProperty rdf:about="http://example.org/onto/prop/google_filestore_backup_capacity_gb">
    <rdfs:label>capacity_gb</rdfs:label>
    <rdfs:comment>The amount of bytes needed to allocate a full copy of the snapshot content.</rdfs:comment>
    <rdfs:domain rdf:resource="http://example.org/onto/class/google_filestore_backup"/>
    <rdfs:range rdf:resource="http://www.w3.org/2001/XMLSchema#string"/>
  </owl:DatatypeProperty>
  <owl:DatatypeProperty rdf:about="http://example.org/onto/prop/google_filestore_backup_create_time">
    <rdfs:label>create_time</rdfs:label>
    <rdfs:comment>The time when the snapshot was created in RFC3339 text format.</rdfs:comment>
    <rdfs:domain rdf:resource="http://example.org/onto/class/google_filestore_backup"/>
    <rdfs:range rdf:resource="http://www.w3.org/2001/XMLSchema#string"/>
  </owl:DatatypeProperty>
  <owl:DatatypeProperty rdf:about="http://example.org/onto/prop/google_filestore_backup_description">
    <rdfs:label>description</rdfs:label>
    <rdfs:comment>A description of the backup with 2048 characters or less. Requests with longer descriptions will be rejected.</rdfs:comment>
    <rdfs:domain rdf:resource="http://example.org/onto/class/google_filestore_backup"/>
    <rdfs:range rdf:resource="http://www.w3.org/2001/XMLSchema#string"/>
  </owl:DatatypeProperty>
  <owl:DatatypeProperty rdf:about="http://example.org/onto/prop/google_filestore_backup_download_bytes">
    <rdfs:label>download_bytes</rdfs:label>
    <rdfs:comment>Amount of bytes that will be downloaded if the backup is restored.</rdfs:comment>
    <rdfs:domain rdf:resource="http://example.org/onto/class/google_filestore_backup"/>
    <rdfs:range rdf:resource="http://www.w3.org/2001/XMLSchema#string"/>
  </owl:DatatypeProperty>
  <owl:DatatypeProperty rdf:about="http://example.org/onto/prop/google_filestore_backup_effective_labels">
    <rdfs:label>effective_labels</rdfs:label>
    <rdfs:comment>All of labels (key/value pairs) present on the resource in GCP, including the labels configured through Terraform, other clients and services.</rdfs:comment>
    <rdfs:domain rdf:resource="http://example.org/onto/class/google_filestore_backup"/>
    <rdfs:range rdf:resource="http://www.w3.org/2001/XMLSchema#string"/>
  </owl:DatatypeProperty>
  <owl:DatatypeProperty rdf:about="http://example.org/onto/prop/google_filestore_backup_id">
    <rdfs:label>id</rdfs:label>
    <rdfs:domain rdf:resource="http://example.org/onto/class/google_filestore_backup"/>
    <rdfs:range rdf:resource="http://www.w3.org/2001/XMLSchema#string"/>
  </owl:DatatypeProperty>
  <owl:DatatypeProperty rdf:about="http://example.org/onto/prop/google_filestore_backup_kms_key_name">
    <rdfs:label>kms_key_name</rdfs:label>
    <rdfs:comment>KMS key name used for data encryption.</rdfs:comment>
    <rdfs:domain rdf:resource="http://example.org/onto/class/google_filestore_backup"/>
    <rdfs:range rdf:resource="http://www.w3.org/2001/XMLSchema#string"/>
  </owl:DatatypeProperty>
  <owl:DatatypeProperty rdf:about="http://example.org/onto/prop/google_filestore_backup_labels">
    <rdfs:label>labels</rdfs:label>
    <rdfs:comment>Resource labels to represent user-provided metadata.


**Note**: This field is non-authoritative, and will only manage the labels present in your configuration.
Please refer to the field 'effective_labels' for all of the labels present on the resource.</rdfs:comment>
    <rdfs:domain rdf:resource="http://example.org/onto/class/google_filestore_backup"/>
    <rdfs:range rdf:resource="http://www.w3.org/2001/XMLSchema#string"/>
  </owl:DatatypeProperty>
  <owl:DatatypeProperty rdf:about="http://example.org/onto/prop/google_filestore_backup_location">
    <rdfs:label>location</rdfs:label>
    <rdfs:comment>The name of the location of the instance. This can be a region for ENTERPRISE tier instances.</rdfs:comment>
    <rdfs:domain rdf:resource="http://example.org/onto/class/google_filestore_backup"/>
    <rdfs:range rdf:resource="http://www.w3.org/2001/XMLSchema#string"/>
  </owl:DatatypeProperty>
  <owl:DatatypeProperty rdf:about="http://example.org/onto/prop/google_filestore_backup_name">
    <rdfs:label>name</rdfs:label>
    <rdfs:comment>The resource name of the backup. The name must be unique within the specified instance.

The name must be 1-63 characters long, and comply with
RFC1035. Specifically, the name must be 1-63 characters long and match
the regular expression '[a-z]([-a-z0-9]*[a-z0-9])?' which means the
first character must be a lowercase letter, and all following
characters must be a dash, lowercase letter, or digit, except the last
character, which cannot be a dash.</rdfs:comment>
    <rdfs:domain rdf:resource="http://example.org/onto/class/google_filestore_backup"/>
    <rdfs:range rdf:resource="http://www.w3.org/2001/XMLSchema#string"/>
  </owl:DatatypeProperty>
  <owl:DatatypeProperty rdf:about="http://example.org/onto/prop/google_filestore_backup_project">
    <rdfs:label>project</rdfs:label>
    <rdfs:domain rdf:resource="http://example.org/onto/class/google_filestore_backup"/>
    <rdfs:range rdf:resource="http://www.w3.org/2001/XMLSchema#string"/>
  </owl:DatatypeProperty>
  <owl:DatatypeProperty rdf:about="http://example.org/onto/prop/google_filestore_backup_source_file_share">
    <rdfs:label>source_file_share</rdfs:label>
    <rdfs:comment>Name of the file share in the source Cloud Filestore instance that the backup is created from.</rdfs:comment>
    <rdfs:domain rdf:resource="http://example.org/onto/class/google_filestore_backup"/>
    <rdfs:range rdf:resource="http://www.w3.org/2001/XMLSchema#string"/>
  </owl:DatatypeProperty>
  <owl:DatatypeProperty rdf:about="http://example.org/onto/prop/google_filestore_backup_source_instance">
    <rdfs:label>source_instance</rdfs:label>
    <rdfs:comment>The resource name of the source Cloud Filestore instance, in the format projects/{projectId}/locations/{locationId}/instances/{instanceId}, used to create this backup.</rdfs:comment>
    <rdfs:domain rdf:resource="http://example.org/onto/class/google_filestore_backup"/>
    <rdfs:range rdf:resource="http://www.w3.org/2001/XMLSchema#string"/>
  </owl:DatatypeProperty>
  <owl:DatatypeProperty rdf:about="http://example.org/onto/prop/google_filestore_backup_source_instance_tier">
    <rdfs:label>source_instance_tier</rdfs:label>
    <rdfs:comment>The service tier of the source Cloud Filestore instance that this backup is created from.</rdfs:comment>
    <rdfs:domain rdf:resource="http://example.org/onto/class/google_filestore_backup"/>
    <rdfs:range rdf:resource="http://www.w3.org/2001/XMLSchema#string"/>
  </owl:DatatypeProperty>
  <owl:DatatypeProperty rdf:about="http://example.org/onto/prop/google_filestore_backup_state">
    <rdfs:label>state</rdfs:label>
    <rdfs:comment>The backup state.</rdfs:comment>
    <rdfs:domain rdf:resource="http://example.org/onto/class/google_filestore_backup"/>
    <rdfs:range rdf:resource="http://www.w3.org/2001/XMLSchema#string"/>
  </owl:DatatypeProperty>
  <owl:DatatypeProperty rdf:about="http://example.org/onto/prop/google_filestore_backup_storage_bytes">
    <rdfs:label>storage_bytes</rdfs:label>
    <rdfs:comment>The size of the storage used by the backup. As backups share storage, this number is expected to change with backup creation/deletion.</rdfs:comment>
    <rdfs:domain rdf:resource="http://example.org/onto/class/google_filestore_backup"/>
    <rdfs:range rdf:resource="http://www.w3.org/2001/XMLSchema#string"/>
  </owl:DatatypeProperty>
  <owl:DatatypeProperty rdf:about="http://example.org/onto/prop/google_filestore_backup_tags">
    <rdfs:label>tags</rdfs:label>
    <rdfs:comment>A map of resource manager tags.
Resource manager tag keys and values have the same definition as resource manager tags.
Keys must be in the format tagKeys/{tag_key_id}, and values are in the format tagValues/{tag_value_id}.
The field is ignored (both PUT & PATCH) when empty.</rdfs:comment>
    <rdfs:domain rdf:resource="http://example.org/onto/class/google_filestore_backup"/>
    <rdfs:range rdf:resource="http://www.w3.org/2001/XMLSchema#string"/>
  </owl:DatatypeProperty>
  <owl:DatatypeProperty rdf:about="http://example.org/onto/prop/google_filestore_backup_terraform_labels">
    <rdfs:label>terraform_labels</rdfs:label>
    <rdfs:comment>The combination of labels configured directly on the resource
 and default labels configured on the provider.</rdfs:comment>
    <rdfs:domain rdf:resource="http://example.org/onto/class/google_filestore_backup"/>
    <rdfs:range rdf:resource="http://www.w3.org/2001/XMLSchema#string"/>
  </owl:DatatypeProperty>
  <owl:DatatypeProperty rdf:about="http://example.org/onto/prop/google_filestore_backup_create">
    <rdfs:label>create</rdfs:label>
    <rdfs:domain rdf:resource="http://example.org/onto/class/google_filestore_backup"/>
    <rdfs:range rdf:resource="http://www.w3.org/2001/XMLSchema#string"/>
  </owl:DatatypeProperty>
  <owl:DatatypeProperty rdf:about="http://example.org/onto/prop/google_filestore_backup_delete">
    <rdfs:label>delete</rdfs:label>
    <rdfs:domain rdf:resource="http://example.org/onto/class/google_filestore_backup"/>
    <rdfs:range rdf:resource="http://www.w3.org/2001/XMLSchema#string"/>
  </owl:DatatypeProperty>
  <owl:DatatypeProperty rdf:about="http://example.org/onto/prop/google_filestore_backup_update">
    <rdfs:label>update</rdfs:label>
    <rdfs:domain rdf:resource="http://example.org/onto/class/google_filestore_backup"/>
    <rdfs:range rdf:resource="http://www.w3.org/2001/XMLSchema#string"/>
  </owl:DatatypeProperty>
</rdf:RDF>
