<?xml version="1.0" encoding="UTF-8"?>
<rdf:RDF
  xmlns:rdf="http://www.w3.org/1999/02/22-rdf-syntax-ns#"
  xmlns:rdfs="http://www.w3.org/2000/01/rdf-schema#"
  xmlns:owl="http://www.w3.org/2002/07/owl#"
  xmlns:xsd="http://www.w3.org/2001/XMLSchema#"
  xml:base="http://example.org/onto/">
  <owl:Class rdf:about="http://example.org/onto/class/google_clouddomains_registration">
    <rdfs:label>google_clouddomains_registration</rdfs:label>
    <rdfs:comment>#
#     ***     AUTO GENERATED CODE    ***    Type: MMv1     ***
#
# ----------------------------------------------------------------------------
#
#     This code is generated by Magic Modules using the following:
#
#     Configuration: https:#github.com/GoogleCloudPlatform/magic-modules/tree/main/mmv1/products/clouddomains/Registration.yaml
#     Template:      https:#github.com/GoogleCloudPlatform/magic-modules/tree/main/mmv1/templates/terraform/resource.html.markdown.tmpl
#
#     DO NOT EDIT this file directly. Any changes made to this file will be
#     overwritten during the next generation cycle.
#
# ----------------------------------------------------------------------------
subcategory: "Cloud Domains"
description: |-
  Registers a new domain name and creates a corresponding Registration resource.
---</rdfs:comment>
  </owl:Class>
  <owl:DatatypeProperty rdf:about="http://example.org/onto/prop/google_clouddomains_registration_contact_notices">
    <rdfs:label>contact_notices</rdfs:label>
    <rdfs:comment>The list of contact notices that the caller acknowledges. Possible value is PUBLIC_CONTACT_DATA_ACKNOWLEDGEMENT</rdfs:comment>
    <rdfs:domain rdf:resource="http://example.org/onto/class/google_clouddomains_registration"/>
    <rdfs:range rdf:resource="http://www.w3.org/2001/XMLSchema#string"/>
  </owl:DatatypeProperty>
  <owl:DatatypeProperty rdf:about="http://example.org/onto/prop/google_clouddomains_registration_create_time">
    <rdfs:label>create_time</rdfs:label>
    <rdfs:comment>Output only. Time at which the automation was created.</rdfs:comment>
    <rdfs:domain rdf:resource="http://example.org/onto/class/google_clouddomains_registration"/>
    <rdfs:range rdf:resource="http://www.w3.org/2001/XMLSchema#string"/>
  </owl:DatatypeProperty>
  <owl:DatatypeProperty rdf:about="http://example.org/onto/prop/google_clouddomains_registration_domain_name">
    <rdfs:label>domain_name</rdfs:label>
    <rdfs:comment>Required. The domain name. Unicode domain names must be expressed in Punycode format.</rdfs:comment>
    <rdfs:domain rdf:resource="http://example.org/onto/class/google_clouddomains_registration"/>
    <rdfs:range rdf:resource="http://www.w3.org/2001/XMLSchema#string"/>
  </owl:DatatypeProperty>
  <owl:DatatypeProperty rdf:about="http://example.org/onto/prop/google_clouddomains_registration_domain_notices">
    <rdfs:label>domain_notices</rdfs:label>
    <rdfs:comment>The list of domain notices that you acknowledge. Possible value is HSTS_PRELOADED</rdfs:comment>
    <rdfs:domain rdf:resource="http://example.org/onto/class/google_clouddomains_registration"/>
    <rdfs:range rdf:resource="http://www.w3.org/2001/XMLSchema#string"/>
  </owl:DatatypeProperty>
  <owl:DatatypeProperty rdf:about="http://example.org/onto/prop/google_clouddomains_registration_effective_labels">
    <rdfs:label>effective_labels</rdfs:label>
    <rdfs:comment>All of labels (key/value pairs) present on the resource in GCP, including the labels configured through Terraform, other clients and services.</rdfs:comment>
    <rdfs:domain rdf:resource="http://example.org/onto/class/google_clouddomains_registration"/>
    <rdfs:range rdf:resource="http://www.w3.org/2001/XMLSchema#string"/>
  </owl:DatatypeProperty>
  <owl:DatatypeProperty rdf:about="http://example.org/onto/prop/google_clouddomains_registration_expire_time">
    <rdfs:label>expire_time</rdfs:label>
    <rdfs:comment>Output only. Time at which the automation was updated.</rdfs:comment>
    <rdfs:domain rdf:resource="http://example.org/onto/class/google_clouddomains_registration"/>
    <rdfs:range rdf:resource="http://www.w3.org/2001/XMLSchema#string"/>
  </owl:DatatypeProperty>
  <owl:DatatypeProperty rdf:about="http://example.org/onto/prop/google_clouddomains_registration_id">
    <rdfs:label>id</rdfs:label>
    <rdfs:domain rdf:resource="http://example.org/onto/class/google_clouddomains_registration"/>
    <rdfs:range rdf:resource="http://www.w3.org/2001/XMLSchema#string"/>
  </owl:DatatypeProperty>
  <owl:DatatypeProperty rdf:about="http://example.org/onto/prop/google_clouddomains_registration_issues">
    <rdfs:label>issues</rdfs:label>
    <rdfs:comment>Output only. The set of issues with the Registration that require attention.</rdfs:comment>
    <rdfs:domain rdf:resource="http://example.org/onto/class/google_clouddomains_registration"/>
    <rdfs:range rdf:resource="http://www.w3.org/2001/XMLSchema#string"/>
  </owl:DatatypeProperty>
  <owl:DatatypeProperty rdf:about="http://example.org/onto/prop/google_clouddomains_registration_labels">
    <rdfs:label>labels</rdfs:label>
    <rdfs:comment>Set of labels associated with the Registration.

**Note**: This field is non-authoritative, and will only manage the labels present in your configuration.
Please refer to the field 'effective_labels' for all of the labels present on the resource.</rdfs:comment>
    <rdfs:domain rdf:resource="http://example.org/onto/class/google_clouddomains_registration"/>
    <rdfs:range rdf:resource="http://www.w3.org/2001/XMLSchema#string"/>
  </owl:DatatypeProperty>
  <owl:DatatypeProperty rdf:about="http://example.org/onto/prop/google_clouddomains_registration_location">
    <rdfs:label>location</rdfs:label>
    <rdfs:comment>The location for the resource</rdfs:comment>
    <rdfs:domain rdf:resource="http://example.org/onto/class/google_clouddomains_registration"/>
    <rdfs:range rdf:resource="http://www.w3.org/2001/XMLSchema#string"/>
  </owl:DatatypeProperty>
  <owl:DatatypeProperty rdf:about="http://example.org/onto/prop/google_clouddomains_registration_name">
    <rdfs:label>name</rdfs:label>
    <rdfs:comment>Output only. Name of the Registration resource, in the format projects/*/locations/*/registrations/<domain_name>.</rdfs:comment>
    <rdfs:domain rdf:resource="http://example.org/onto/class/google_clouddomains_registration"/>
    <rdfs:range rdf:resource="http://www.w3.org/2001/XMLSchema#string"/>
  </owl:DatatypeProperty>
  <owl:DatatypeProperty rdf:about="http://example.org/onto/prop/google_clouddomains_registration_project">
    <rdfs:label>project</rdfs:label>
    <rdfs:domain rdf:resource="http://example.org/onto/class/google_clouddomains_registration"/>
    <rdfs:range rdf:resource="http://www.w3.org/2001/XMLSchema#string"/>
  </owl:DatatypeProperty>
  <owl:DatatypeProperty rdf:about="http://example.org/onto/prop/google_clouddomains_registration_register_failure_reason">
    <rdfs:label>register_failure_reason</rdfs:label>
    <rdfs:comment>Output only. The reason the domain registration failed. Only set for domains in REGISTRATION_FAILED state.</rdfs:comment>
    <rdfs:domain rdf:resource="http://example.org/onto/class/google_clouddomains_registration"/>
    <rdfs:range rdf:resource="http://www.w3.org/2001/XMLSchema#string"/>
  </owl:DatatypeProperty>
  <owl:DatatypeProperty rdf:about="http://example.org/onto/prop/google_clouddomains_registration_state">
    <rdfs:label>state</rdfs:label>
    <rdfs:comment>Output only. The current state of the Registration.</rdfs:comment>
    <rdfs:domain rdf:resource="http://example.org/onto/class/google_clouddomains_registration"/>
    <rdfs:range rdf:resource="http://www.w3.org/2001/XMLSchema#string"/>
  </owl:DatatypeProperty>
  <owl:DatatypeProperty rdf:about="http://example.org/onto/prop/google_clouddomains_registration_supported_privacy">
    <rdfs:label>supported_privacy</rdfs:label>
    <rdfs:comment>Output only. Set of options for the contactSettings.privacy field that this Registration supports.</rdfs:comment>
    <rdfs:domain rdf:resource="http://example.org/onto/class/google_clouddomains_registration"/>
    <rdfs:range rdf:resource="http://www.w3.org/2001/XMLSchema#string"/>
  </owl:DatatypeProperty>
  <owl:DatatypeProperty rdf:about="http://example.org/onto/prop/google_clouddomains_registration_terraform_labels">
    <rdfs:label>terraform_labels</rdfs:label>
    <rdfs:comment>The combination of labels configured directly on the resource
 and default labels configured on the provider.</rdfs:comment>
    <rdfs:domain rdf:resource="http://example.org/onto/class/google_clouddomains_registration"/>
    <rdfs:range rdf:resource="http://www.w3.org/2001/XMLSchema#string"/>
  </owl:DatatypeProperty>
  <owl:DatatypeProperty rdf:about="http://example.org/onto/prop/google_clouddomains_registration_privacy">
    <rdfs:label>privacy</rdfs:label>
    <rdfs:comment>Required. Privacy setting for the contacts associated with the Registration.
Values are PUBLIC_CONTACT_DATA, PRIVATE_CONTACT_DATA, and REDACTED_CONTACT_DATA</rdfs:comment>
    <rdfs:domain rdf:resource="http://example.org/onto/class/google_clouddomains_registration"/>
    <rdfs:range rdf:resource="http://www.w3.org/2001/XMLSchema#string"/>
  </owl:DatatypeProperty>
  <owl:DatatypeProperty rdf:about="http://example.org/onto/prop/google_clouddomains_registration_email">
    <rdfs:label>email</rdfs:label>
    <rdfs:comment>Required. Email address of the contact.</rdfs:comment>
    <rdfs:domain rdf:resource="http://example.org/onto/class/google_clouddomains_registration"/>
    <rdfs:range rdf:resource="http://www.w3.org/2001/XMLSchema#string"/>
  </owl:DatatypeProperty>
  <owl:DatatypeProperty rdf:about="http://example.org/onto/prop/google_clouddomains_registration_fax_number">
    <rdfs:label>fax_number</rdfs:label>
    <rdfs:comment>Fax number of the contact in international format. For example, "+1-800-555-0123".</rdfs:comment>
    <rdfs:domain rdf:resource="http://example.org/onto/class/google_clouddomains_registration"/>
    <rdfs:range rdf:resource="http://www.w3.org/2001/XMLSchema#string"/>
  </owl:DatatypeProperty>
  <owl:DatatypeProperty rdf:about="http://example.org/onto/prop/google_clouddomains_registration_phone_number">
    <rdfs:label>phone_number</rdfs:label>
    <rdfs:comment>Required. Phone number of the contact in international format. For example, "+1-800-555-0123".</rdfs:comment>
    <rdfs:domain rdf:resource="http://example.org/onto/class/google_clouddomains_registration"/>
    <rdfs:range rdf:resource="http://www.w3.org/2001/XMLSchema#string"/>
  </owl:DatatypeProperty>
  <owl:DatatypeProperty rdf:about="http://example.org/onto/prop/google_clouddomains_registration_address_lines">
    <rdfs:label>address_lines</rdfs:label>
    <rdfs:comment>Unstructured address lines describing the lower levels of an address.
Because values in addressLines do not have type information and may sometimes contain multiple values in a single
field (e.g. "Austin, TX"), it is important that the line order is clear. The order of address lines should be
"envelope order" for the country/region of the address. In places where this can vary (e.g. Japan), address_language
is used to make it explicit (e.g. "ja" for large-to-small ordering and "ja-Latn" or "en" for small-to-large). This way,
the most specific line of an address can be selected based on the language.</rdfs:comment>
    <rdfs:domain rdf:resource="http://example.org/onto/class/google_clouddomains_registration"/>
    <rdfs:range rdf:resource="http://www.w3.org/2001/XMLSchema#string"/>
  </owl:DatatypeProperty>
  <owl:DatatypeProperty rdf:about="http://example.org/onto/prop/google_clouddomains_registration_administrative_area">
    <rdfs:label>administrative_area</rdfs:label>
    <rdfs:comment>Highest administrative subdivision which is used for postal addresses of a country or region. For example, this can be a state,
a province, an oblast, or a prefecture. Specifically, for Spain this is the province and not the autonomous community
(e.g. "Barcelona" and not "Catalonia"). Many countries don't use an administrative area in postal addresses. E.g. in Switzerland
this should be left unpopulated.</rdfs:comment>
    <rdfs:domain rdf:resource="http://example.org/onto/class/google_clouddomains_registration"/>
    <rdfs:range rdf:resource="http://www.w3.org/2001/XMLSchema#string"/>
  </owl:DatatypeProperty>
  <owl:DatatypeProperty rdf:about="http://example.org/onto/prop/google_clouddomains_registration_locality">
    <rdfs:label>locality</rdfs:label>
    <rdfs:comment>Generally refers to the city/town portion of the address. Examples: US city, IT comune, UK post town. In regions of the world
where localities are not well defined or do not fit into this structure well, leave locality empty and use addressLines.</rdfs:comment>
    <rdfs:domain rdf:resource="http://example.org/onto/class/google_clouddomains_registration"/>
    <rdfs:range rdf:resource="http://www.w3.org/2001/XMLSchema#string"/>
  </owl:DatatypeProperty>
  <owl:DatatypeProperty rdf:about="http://example.org/onto/prop/google_clouddomains_registration_organization">
    <rdfs:label>organization</rdfs:label>
    <rdfs:comment>The name of the organization at the address.</rdfs:comment>
    <rdfs:domain rdf:resource="http://example.org/onto/class/google_clouddomains_registration"/>
    <rdfs:range rdf:resource="http://www.w3.org/2001/XMLSchema#string"/>
  </owl:DatatypeProperty>
  <owl:DatatypeProperty rdf:about="http://example.org/onto/prop/google_clouddomains_registration_postal_code">
    <rdfs:label>postal_code</rdfs:label>
    <rdfs:comment>Postal code of the address. Not all countries use or require postal codes to be present, but where they are used,
they may trigger additional validation with other parts of the address (e.g. state/zip validation in the U.S.A.).</rdfs:comment>
    <rdfs:domain rdf:resource="http://example.org/onto/class/google_clouddomains_registration"/>
    <rdfs:range rdf:resource="http://www.w3.org/2001/XMLSchema#string"/>
  </owl:DatatypeProperty>
  <owl:DatatypeProperty rdf:about="http://example.org/onto/prop/google_clouddomains_registration_recipients">
    <rdfs:label>recipients</rdfs:label>
    <rdfs:comment>The recipient at the address. This field may, under certain circumstances, contain multiline information. For example,
it might contain "care of" information.</rdfs:comment>
    <rdfs:domain rdf:resource="http://example.org/onto/class/google_clouddomains_registration"/>
    <rdfs:range rdf:resource="http://www.w3.org/2001/XMLSchema#string"/>
  </owl:DatatypeProperty>
  <owl:DatatypeProperty rdf:about="http://example.org/onto/prop/google_clouddomains_registration_region_code">
    <rdfs:label>region_code</rdfs:label>
    <rdfs:comment>Required. CLDR region code of the country/region of the address. This is never inferred and it is up to the user to
ensure the value is correct. See https://cldr.unicode.org/ and
https://www.unicode.org/cldr/charts/30/supplemental/territory_information.html for details. Example: "CH" for Switzerland.</rdfs:comment>
    <rdfs:domain rdf:resource="http://example.org/onto/class/google_clouddomains_registration"/>
    <rdfs:range rdf:resource="http://www.w3.org/2001/XMLSchema#string"/>
  </owl:DatatypeProperty>
  <owl:DatatypeProperty rdf:about="http://example.org/onto/prop/google_clouddomains_registration_email">
    <rdfs:label>email</rdfs:label>
    <rdfs:comment>Required. Email address of the contact.</rdfs:comment>
    <rdfs:domain rdf:resource="http://example.org/onto/class/google_clouddomains_registration"/>
    <rdfs:range rdf:resource="http://www.w3.org/2001/XMLSchema#string"/>
  </owl:DatatypeProperty>
  <owl:DatatypeProperty rdf:about="http://example.org/onto/prop/google_clouddomains_registration_fax_number">
    <rdfs:label>fax_number</rdfs:label>
    <rdfs:comment>Fax number of the contact in international format. For example, "+1-800-555-0123".</rdfs:comment>
    <rdfs:domain rdf:resource="http://example.org/onto/class/google_clouddomains_registration"/>
    <rdfs:range rdf:resource="http://www.w3.org/2001/XMLSchema#string"/>
  </owl:DatatypeProperty>
  <owl:DatatypeProperty rdf:about="http://example.org/onto/prop/google_clouddomains_registration_phone_number">
    <rdfs:label>phone_number</rdfs:label>
    <rdfs:comment>Required. Phone number of the contact in international format. For example, "+1-800-555-0123".</rdfs:comment>
    <rdfs:domain rdf:resource="http://example.org/onto/class/google_clouddomains_registration"/>
    <rdfs:range rdf:resource="http://www.w3.org/2001/XMLSchema#string"/>
  </owl:DatatypeProperty>
  <owl:DatatypeProperty rdf:about="http://example.org/onto/prop/google_clouddomains_registration_address_lines">
    <rdfs:label>address_lines</rdfs:label>
    <rdfs:comment>Unstructured address lines describing the lower levels of an address.
Because values in addressLines do not have type information and may sometimes contain multiple values in a single
field (e.g. "Austin, TX"), it is important that the line order is clear. The order of address lines should be
"envelope order" for the country/region of the address. In places where this can vary (e.g. Japan), address_language
is used to make it explicit (e.g. "ja" for large-to-small ordering and "ja-Latn" or "en" for small-to-large). This way,
the most specific line of an address can be selected based on the language.</rdfs:comment>
    <rdfs:domain rdf:resource="http://example.org/onto/class/google_clouddomains_registration"/>
    <rdfs:range rdf:resource="http://www.w3.org/2001/XMLSchema#string"/>
  </owl:DatatypeProperty>
  <owl:DatatypeProperty rdf:about="http://example.org/onto/prop/google_clouddomains_registration_administrative_area">
    <rdfs:label>administrative_area</rdfs:label>
    <rdfs:comment>Highest administrative subdivision which is used for postal addresses of a country or region. For example, this can be a state,
a province, an oblast, or a prefecture. Specifically, for Spain this is the province and not the autonomous community
(e.g. "Barcelona" and not "Catalonia"). Many countries don't use an administrative area in postal addresses. E.g. in Switzerland
this should be left unpopulated.</rdfs:comment>
    <rdfs:domain rdf:resource="http://example.org/onto/class/google_clouddomains_registration"/>
    <rdfs:range rdf:resource="http://www.w3.org/2001/XMLSchema#string"/>
  </owl:DatatypeProperty>
  <owl:DatatypeProperty rdf:about="http://example.org/onto/prop/google_clouddomains_registration_locality">
    <rdfs:label>locality</rdfs:label>
    <rdfs:comment>Generally refers to the city/town portion of the address. Examples: US city, IT comune, UK post town. In regions of the world
where localities are not well defined or do not fit into this structure well, leave locality empty and use addressLines.</rdfs:comment>
    <rdfs:domain rdf:resource="http://example.org/onto/class/google_clouddomains_registration"/>
    <rdfs:range rdf:resource="http://www.w3.org/2001/XMLSchema#string"/>
  </owl:DatatypeProperty>
  <owl:DatatypeProperty rdf:about="http://example.org/onto/prop/google_clouddomains_registration_organization">
    <rdfs:label>organization</rdfs:label>
    <rdfs:comment>The name of the organization at the address.</rdfs:comment>
    <rdfs:domain rdf:resource="http://example.org/onto/class/google_clouddomains_registration"/>
    <rdfs:range rdf:resource="http://www.w3.org/2001/XMLSchema#string"/>
  </owl:DatatypeProperty>
  <owl:DatatypeProperty rdf:about="http://example.org/onto/prop/google_clouddomains_registration_postal_code">
    <rdfs:label>postal_code</rdfs:label>
    <rdfs:comment>Postal code of the address. Not all countries use or require postal codes to be present, but where they are used,
they may trigger additional validation with other parts of the address (e.g. state/zip validation in the U.S.A.).</rdfs:comment>
    <rdfs:domain rdf:resource="http://example.org/onto/class/google_clouddomains_registration"/>
    <rdfs:range rdf:resource="http://www.w3.org/2001/XMLSchema#string"/>
  </owl:DatatypeProperty>
  <owl:DatatypeProperty rdf:about="http://example.org/onto/prop/google_clouddomains_registration_recipients">
    <rdfs:label>recipients</rdfs:label>
    <rdfs:comment>The recipient at the address. This field may, under certain circumstances, contain multiline information. For example,
it might contain "care of" information.</rdfs:comment>
    <rdfs:domain rdf:resource="http://example.org/onto/class/google_clouddomains_registration"/>
    <rdfs:range rdf:resource="http://www.w3.org/2001/XMLSchema#string"/>
  </owl:DatatypeProperty>
  <owl:DatatypeProperty rdf:about="http://example.org/onto/prop/google_clouddomains_registration_region_code">
    <rdfs:label>region_code</rdfs:label>
    <rdfs:comment>Required. CLDR region code of the country/region of the address. This is never inferred and it is up to the user to
ensure the value is correct. See https://cldr.unicode.org/ and
https://www.unicode.org/cldr/charts/30/supplemental/territory_information.html for details. Example: "CH" for Switzerland.</rdfs:comment>
    <rdfs:domain rdf:resource="http://example.org/onto/class/google_clouddomains_registration"/>
    <rdfs:range rdf:resource="http://www.w3.org/2001/XMLSchema#string"/>
  </owl:DatatypeProperty>
  <owl:DatatypeProperty rdf:about="http://example.org/onto/prop/google_clouddomains_registration_email">
    <rdfs:label>email</rdfs:label>
    <rdfs:comment>Required. Email address of the contact.</rdfs:comment>
    <rdfs:domain rdf:resource="http://example.org/onto/class/google_clouddomains_registration"/>
    <rdfs:range rdf:resource="http://www.w3.org/2001/XMLSchema#string"/>
  </owl:DatatypeProperty>
  <owl:DatatypeProperty rdf:about="http://example.org/onto/prop/google_clouddomains_registration_fax_number">
    <rdfs:label>fax_number</rdfs:label>
    <rdfs:comment>Fax number of the contact in international format. For example, "+1-800-555-0123".</rdfs:comment>
    <rdfs:domain rdf:resource="http://example.org/onto/class/google_clouddomains_registration"/>
    <rdfs:range rdf:resource="http://www.w3.org/2001/XMLSchema#string"/>
  </owl:DatatypeProperty>
  <owl:DatatypeProperty rdf:about="http://example.org/onto/prop/google_clouddomains_registration_phone_number">
    <rdfs:label>phone_number</rdfs:label>
    <rdfs:comment>Required. Phone number of the contact in international format. For example, "+1-800-555-0123".</rdfs:comment>
    <rdfs:domain rdf:resource="http://example.org/onto/class/google_clouddomains_registration"/>
    <rdfs:range rdf:resource="http://www.w3.org/2001/XMLSchema#string"/>
  </owl:DatatypeProperty>
  <owl:DatatypeProperty rdf:about="http://example.org/onto/prop/google_clouddomains_registration_address_lines">
    <rdfs:label>address_lines</rdfs:label>
    <rdfs:comment>Unstructured address lines describing the lower levels of an address.
Because values in addressLines do not have type information and may sometimes contain multiple values in a single
field (e.g. "Austin, TX"), it is important that the line order is clear. The order of address lines should be
"envelope order" for the country/region of the address. In places where this can vary (e.g. Japan), address_language
is used to make it explicit (e.g. "ja" for large-to-small ordering and "ja-Latn" or "en" for small-to-large). This way,
the most specific line of an address can be selected based on the language.</rdfs:comment>
    <rdfs:domain rdf:resource="http://example.org/onto/class/google_clouddomains_registration"/>
    <rdfs:range rdf:resource="http://www.w3.org/2001/XMLSchema#string"/>
  </owl:DatatypeProperty>
  <owl:DatatypeProperty rdf:about="http://example.org/onto/prop/google_clouddomains_registration_administrative_area">
    <rdfs:label>administrative_area</rdfs:label>
    <rdfs:comment>Highest administrative subdivision which is used for postal addresses of a country or region. For example, this can be a state,
a province, an oblast, or a prefecture. Specifically, for Spain this is the province and not the autonomous community
(e.g. "Barcelona" and not "Catalonia"). Many countries don't use an administrative area in postal addresses. E.g. in Switzerland
this should be left unpopulated.</rdfs:comment>
    <rdfs:domain rdf:resource="http://example.org/onto/class/google_clouddomains_registration"/>
    <rdfs:range rdf:resource="http://www.w3.org/2001/XMLSchema#string"/>
  </owl:DatatypeProperty>
  <owl:DatatypeProperty rdf:about="http://example.org/onto/prop/google_clouddomains_registration_locality">
    <rdfs:label>locality</rdfs:label>
    <rdfs:comment>Generally refers to the city/town portion of the address. Examples: US city, IT comune, UK post town. In regions of the world
where localities are not well defined or do not fit into this structure well, leave locality empty and use addressLines.</rdfs:comment>
    <rdfs:domain rdf:resource="http://example.org/onto/class/google_clouddomains_registration"/>
    <rdfs:range rdf:resource="http://www.w3.org/2001/XMLSchema#string"/>
  </owl:DatatypeProperty>
  <owl:DatatypeProperty rdf:about="http://example.org/onto/prop/google_clouddomains_registration_organization">
    <rdfs:label>organization</rdfs:label>
    <rdfs:comment>The name of the organization at the address.</rdfs:comment>
    <rdfs:domain rdf:resource="http://example.org/onto/class/google_clouddomains_registration"/>
    <rdfs:range rdf:resource="http://www.w3.org/2001/XMLSchema#string"/>
  </owl:DatatypeProperty>
  <owl:DatatypeProperty rdf:about="http://example.org/onto/prop/google_clouddomains_registration_postal_code">
    <rdfs:label>postal_code</rdfs:label>
    <rdfs:comment>Postal code of the address. Not all countries use or require postal codes to be present, but where they are used,
they may trigger additional validation with other parts of the address (e.g. state/zip validation in the U.S.A.).</rdfs:comment>
    <rdfs:domain rdf:resource="http://example.org/onto/class/google_clouddomains_registration"/>
    <rdfs:range rdf:resource="http://www.w3.org/2001/XMLSchema#string"/>
  </owl:DatatypeProperty>
  <owl:DatatypeProperty rdf:about="http://example.org/onto/prop/google_clouddomains_registration_recipients">
    <rdfs:label>recipients</rdfs:label>
    <rdfs:comment>The recipient at the address. This field may, under certain circumstances, contain multiline information. For example,
it might contain "care of" information.</rdfs:comment>
    <rdfs:domain rdf:resource="http://example.org/onto/class/google_clouddomains_registration"/>
    <rdfs:range rdf:resource="http://www.w3.org/2001/XMLSchema#string"/>
  </owl:DatatypeProperty>
  <owl:DatatypeProperty rdf:about="http://example.org/onto/prop/google_clouddomains_registration_region_code">
    <rdfs:label>region_code</rdfs:label>
    <rdfs:comment>Required. CLDR region code of the country/region of the address. This is never inferred and it is up to the user to
ensure the value is correct. See https://cldr.unicode.org/ and
https://www.unicode.org/cldr/charts/30/supplemental/territory_information.html for details. Example: "CH" for Switzerland.</rdfs:comment>
    <rdfs:domain rdf:resource="http://example.org/onto/class/google_clouddomains_registration"/>
    <rdfs:range rdf:resource="http://www.w3.org/2001/XMLSchema#string"/>
  </owl:DatatypeProperty>
  <owl:DatatypeProperty rdf:about="http://example.org/onto/prop/google_clouddomains_registration_name_servers">
    <rdfs:label>name_servers</rdfs:label>
    <rdfs:comment>Required. A list of name servers that store the DNS zone for this domain. Each name server is a domain
name, with Unicode domain names expressed in Punycode format.</rdfs:comment>
    <rdfs:domain rdf:resource="http://example.org/onto/class/google_clouddomains_registration"/>
    <rdfs:range rdf:resource="http://www.w3.org/2001/XMLSchema#string"/>
  </owl:DatatypeProperty>
  <owl:DatatypeProperty rdf:about="http://example.org/onto/prop/google_clouddomains_registration_algorithm">
    <rdfs:label>algorithm</rdfs:label>
    <rdfs:comment>The algorithm used to generate the referenced DNSKEY.</rdfs:comment>
    <rdfs:domain rdf:resource="http://example.org/onto/class/google_clouddomains_registration"/>
    <rdfs:range rdf:resource="http://www.w3.org/2001/XMLSchema#string"/>
  </owl:DatatypeProperty>
  <owl:DatatypeProperty rdf:about="http://example.org/onto/prop/google_clouddomains_registration_digest">
    <rdfs:label>digest</rdfs:label>
    <rdfs:comment>The digest generated from the referenced DNSKEY.</rdfs:comment>
    <rdfs:domain rdf:resource="http://example.org/onto/class/google_clouddomains_registration"/>
    <rdfs:range rdf:resource="http://www.w3.org/2001/XMLSchema#string"/>
  </owl:DatatypeProperty>
  <owl:DatatypeProperty rdf:about="http://example.org/onto/prop/google_clouddomains_registration_digest_type">
    <rdfs:label>digest_type</rdfs:label>
    <rdfs:comment>The hash function used to generate the digest of the referenced DNSKEY.</rdfs:comment>
    <rdfs:domain rdf:resource="http://example.org/onto/class/google_clouddomains_registration"/>
    <rdfs:range rdf:resource="http://www.w3.org/2001/XMLSchema#string"/>
  </owl:DatatypeProperty>
  <owl:DatatypeProperty rdf:about="http://example.org/onto/prop/google_clouddomains_registration_key_tag">
    <rdfs:label>key_tag</rdfs:label>
    <rdfs:comment>The key tag of the record. Must be set in range 0 -- 65535.</rdfs:comment>
    <rdfs:domain rdf:resource="http://example.org/onto/class/google_clouddomains_registration"/>
    <rdfs:range rdf:resource="http://www.w3.org/2001/XMLSchema#string"/>
  </owl:DatatypeProperty>
  <owl:DatatypeProperty rdf:about="http://example.org/onto/prop/google_clouddomains_registration_host_name">
    <rdfs:label>host_name</rdfs:label>
    <rdfs:comment>Required. Domain name of the host in Punycode format.</rdfs:comment>
    <rdfs:domain rdf:resource="http://example.org/onto/class/google_clouddomains_registration"/>
    <rdfs:range rdf:resource="http://www.w3.org/2001/XMLSchema#string"/>
  </owl:DatatypeProperty>
  <owl:DatatypeProperty rdf:about="http://example.org/onto/prop/google_clouddomains_registration_ipv4_addresses">
    <rdfs:label>ipv4_addresses</rdfs:label>
    <rdfs:comment>List of IPv4 addresses corresponding to this host in the standard decimal format (e.g. 198.51.100.1).
At least one of ipv4_address and ipv6_address must be set.</rdfs:comment>
    <rdfs:domain rdf:resource="http://example.org/onto/class/google_clouddomains_registration"/>
    <rdfs:range rdf:resource="http://www.w3.org/2001/XMLSchema#string"/>
  </owl:DatatypeProperty>
  <owl:DatatypeProperty rdf:about="http://example.org/onto/prop/google_clouddomains_registration_ipv6_addresses">
    <rdfs:label>ipv6_addresses</rdfs:label>
    <rdfs:comment>List of IPv4 addresses corresponding to this host in the standard decimal format (e.g. 198.51.100.1).
At least one of ipv4_address and ipv6_address must be set.</rdfs:comment>
    <rdfs:domain rdf:resource="http://example.org/onto/class/google_clouddomains_registration"/>
    <rdfs:range rdf:resource="http://www.w3.org/2001/XMLSchema#string"/>
  </owl:DatatypeProperty>
  <owl:DatatypeProperty rdf:about="http://example.org/onto/prop/google_clouddomains_registration_preferred_renewal_method">
    <rdfs:label>preferred_renewal_method</rdfs:label>
    <rdfs:comment>The desired renewal method for this Registration. The actual renewalMethod is automatically updated to reflect this choice.
If unset or equal to RENEWAL_METHOD_UNSPECIFIED, the actual renewalMethod is treated as if it were set to AUTOMATIC_RENEWAL.
You cannot use RENEWAL_DISABLED during resource creation, and you can update the renewal status only when the Registration
resource has state ACTIVE or SUSPENDED.

When preferredRenewalMethod is set to AUTOMATIC_RENEWAL, the actual renewalMethod can be set to RENEWAL_DISABLED in case of
problems with the billing account or reported domain abuse. In such cases, check the issues field on the Registration. After
the problem is resolved, the renewalMethod is automatically updated to preferredRenewalMethod in a few hours.</rdfs:comment>
    <rdfs:domain rdf:resource="http://example.org/onto/class/google_clouddomains_registration"/>
    <rdfs:range rdf:resource="http://www.w3.org/2001/XMLSchema#string"/>
  </owl:DatatypeProperty>
  <owl:DatatypeProperty rdf:about="http://example.org/onto/prop/google_clouddomains_registration_renewal_method">
    <rdfs:label>renewal_method</rdfs:label>
    <rdfs:comment>Output only. The actual renewal method for this Registration. When preferredRenewalMethod is set to AUTOMATIC_RENEWAL,
the actual renewalMethod can be equal to RENEWAL_DISABLED—for example, when there are problems with the billing account
or reported domain abuse. In such cases, check the issues field on the Registration. After the problem is resolved, the
renewalMethod is automatically updated to preferredRenewalMethod in a few hours.</rdfs:comment>
    <rdfs:domain rdf:resource="http://example.org/onto/class/google_clouddomains_registration"/>
    <rdfs:range rdf:resource="http://www.w3.org/2001/XMLSchema#string"/>
  </owl:DatatypeProperty>
  <owl:DatatypeProperty rdf:about="http://example.org/onto/prop/google_clouddomains_registration_transfer_lock_state">
    <rdfs:label>transfer_lock_state</rdfs:label>
    <rdfs:comment>Controls whether the domain can be transferred to another registrar. Values are UNLOCKED or LOCKED.</rdfs:comment>
    <rdfs:domain rdf:resource="http://example.org/onto/class/google_clouddomains_registration"/>
    <rdfs:range rdf:resource="http://www.w3.org/2001/XMLSchema#string"/>
  </owl:DatatypeProperty>
  <owl:DatatypeProperty rdf:about="http://example.org/onto/prop/google_clouddomains_registration_create">
    <rdfs:label>create</rdfs:label>
    <rdfs:domain rdf:resource="http://example.org/onto/class/google_clouddomains_registration"/>
    <rdfs:range rdf:resource="http://www.w3.org/2001/XMLSchema#string"/>
  </owl:DatatypeProperty>
  <owl:DatatypeProperty rdf:about="http://example.org/onto/prop/google_clouddomains_registration_delete">
    <rdfs:label>delete</rdfs:label>
    <rdfs:domain rdf:resource="http://example.org/onto/class/google_clouddomains_registration"/>
    <rdfs:range rdf:resource="http://www.w3.org/2001/XMLSchema#string"/>
  </owl:DatatypeProperty>
  <owl:DatatypeProperty rdf:about="http://example.org/onto/prop/google_clouddomains_registration_update">
    <rdfs:label>update</rdfs:label>
    <rdfs:domain rdf:resource="http://example.org/onto/class/google_clouddomains_registration"/>
    <rdfs:range rdf:resource="http://www.w3.org/2001/XMLSchema#string"/>
  </owl:DatatypeProperty>
  <owl:DatatypeProperty rdf:about="http://example.org/onto/prop/google_clouddomains_registration_currency_code">
    <rdfs:label>currency_code</rdfs:label>
    <rdfs:comment>The three-letter currency code defined in ISO 4217.</rdfs:comment>
    <rdfs:domain rdf:resource="http://example.org/onto/class/google_clouddomains_registration"/>
    <rdfs:range rdf:resource="http://www.w3.org/2001/XMLSchema#string"/>
  </owl:DatatypeProperty>
  <owl:DatatypeProperty rdf:about="http://example.org/onto/prop/google_clouddomains_registration_units">
    <rdfs:label>units</rdfs:label>
    <rdfs:comment>The whole units of the amount. For example if currencyCode is "USD", then 1 unit is one US dollar.</rdfs:comment>
    <rdfs:domain rdf:resource="http://example.org/onto/class/google_clouddomains_registration"/>
    <rdfs:range rdf:resource="http://www.w3.org/2001/XMLSchema#string"/>
  </owl:DatatypeProperty>
</rdf:RDF>
