<?xml version="1.0" encoding="UTF-8"?>
<rdf:RDF
  xmlns:rdf="http://www.w3.org/1999/02/22-rdf-syntax-ns#"
  xmlns:rdfs="http://www.w3.org/2000/01/rdf-schema#"
  xmlns:owl="http://www.w3.org/2002/07/owl#"
  xmlns:xsd="http://www.w3.org/2001/XMLSchema#"
  xml:base="http://example.org/onto/">
  <owl:Class rdf:about="http://example.org/onto/class/google_apigee_api_deployment">
    <rdfs:label>google_apigee_api_deployment</rdfs:label>
    <rdfs:comment>#
#     ***     AUTO GENERATED CODE    ***    Type: MMv1     ***
#
# ----------------------------------------------------------------------------
#
#     This code is generated by Magic Modules using the following:
#
#     Configuration: https:#github.com/GoogleCloudPlatform/magic-modules/tree/main/mmv1/products/apigee/ApiDeployment.yaml
#     Template:      https:#github.com/GoogleCloudPlatform/magic-modules/tree/main/mmv1/templates/terraform/resource.html.markdown.tmpl
#
#     DO NOT EDIT this file directly. Any changes made to this file will be
#     overwritten during the next generation cycle.
#
# ----------------------------------------------------------------------------
subcategory: "Apigee"
description: |-
  Manages a deployment of an API proxy.
---</rdfs:comment>
  </owl:Class>
  <owl:DatatypeProperty rdf:about="http://example.org/onto/prop/google_apigee_api_deployment_environment">
    <rdfs:label>environment</rdfs:label>
    <rdfs:comment>The Apigee Environment associated with the Apigee API deployment.</rdfs:comment>
    <rdfs:domain rdf:resource="http://example.org/onto/class/google_apigee_api_deployment"/>
    <rdfs:range rdf:resource="http://www.w3.org/2001/XMLSchema#string"/>
  </owl:DatatypeProperty>
  <owl:DatatypeProperty rdf:about="http://example.org/onto/prop/google_apigee_api_deployment_id">
    <rdfs:label>id</rdfs:label>
    <rdfs:comment>The ID of the API deployment in the format 'organizations/{{org_id}}/environments/{{environment}}/apis/{{proxy_id}}/revisions/{{revision}}/deployments'.</rdfs:comment>
    <rdfs:domain rdf:resource="http://example.org/onto/class/google_apigee_api_deployment"/>
    <rdfs:range rdf:resource="http://www.w3.org/2001/XMLSchema#string"/>
  </owl:DatatypeProperty>
  <owl:DatatypeProperty rdf:about="http://example.org/onto/prop/google_apigee_api_deployment_org_id">
    <rdfs:label>org_id</rdfs:label>
    <rdfs:comment>The Apigee Organization associated with the Apigee API deployment.</rdfs:comment>
    <rdfs:domain rdf:resource="http://example.org/onto/class/google_apigee_api_deployment"/>
    <rdfs:range rdf:resource="http://www.w3.org/2001/XMLSchema#string"/>
  </owl:DatatypeProperty>
  <owl:DatatypeProperty rdf:about="http://example.org/onto/prop/google_apigee_api_deployment_proxy_id">
    <rdfs:label>proxy_id</rdfs:label>
    <rdfs:comment>The Apigee API associated with the Apigee API deployment.</rdfs:comment>
    <rdfs:domain rdf:resource="http://example.org/onto/class/google_apigee_api_deployment"/>
    <rdfs:range rdf:resource="http://www.w3.org/2001/XMLSchema#string"/>
  </owl:DatatypeProperty>
  <owl:DatatypeProperty rdf:about="http://example.org/onto/prop/google_apigee_api_deployment_revision">
    <rdfs:label>revision</rdfs:label>
    <rdfs:comment>The revision of the API proxy to be deployed.</rdfs:comment>
    <rdfs:domain rdf:resource="http://example.org/onto/class/google_apigee_api_deployment"/>
    <rdfs:range rdf:resource="http://www.w3.org/2001/XMLSchema#string"/>
  </owl:DatatypeProperty>
  <owl:DatatypeProperty rdf:about="http://example.org/onto/prop/google_apigee_api_deployment_create">
    <rdfs:label>create</rdfs:label>
    <rdfs:domain rdf:resource="http://example.org/onto/class/google_apigee_api_deployment"/>
    <rdfs:range rdf:resource="http://www.w3.org/2001/XMLSchema#string"/>
  </owl:DatatypeProperty>
  <owl:DatatypeProperty rdf:about="http://example.org/onto/prop/google_apigee_api_deployment_delete">
    <rdfs:label>delete</rdfs:label>
    <rdfs:domain rdf:resource="http://example.org/onto/class/google_apigee_api_deployment"/>
    <rdfs:range rdf:resource="http://www.w3.org/2001/XMLSchema#string"/>
  </owl:DatatypeProperty>
</rdf:RDF>
