<?xml version="1.0" encoding="UTF-8"?>
<rdf:RDF
  xmlns:rdf="http://www.w3.org/1999/02/22-rdf-syntax-ns#"
  xmlns:rdfs="http://www.w3.org/2000/01/rdf-schema#"
  xmlns:owl="http://www.w3.org/2002/07/owl#"
  xmlns:xsd="http://www.w3.org/2001/XMLSchema#"
  xml:base="http://example.org/onto/">
  <owl:Class rdf:about="http://example.org/onto/class/google_developer_connect_connection">
    <rdfs:label>google_developer_connect_connection</rdfs:label>
    <rdfs:comment>#
#     ***     AUTO GENERATED CODE    ***    Type: MMv1     ***
#
# ----------------------------------------------------------------------------
#
#     This code is generated by Magic Modules using the following:
#
#     Configuration: https:#github.com/GoogleCloudPlatform/magic-modules/tree/main/mmv1/products/developerconnect/Connection.yaml
#     Template:      https:#github.com/GoogleCloudPlatform/magic-modules/tree/main/mmv1/templates/terraform/resource.html.markdown.tmpl
#
#     DO NOT EDIT this file directly. Any changes made to this file will be
#     overwritten during the next generation cycle.
#
# ----------------------------------------------------------------------------
subcategory: "Developer Connect"
description: |-
  A connection for GitHub, GitHub Enterprise, GitLab, and GitLab Enterprise.
---</rdfs:comment>
  </owl:Class>
  <owl:DatatypeProperty rdf:about="http://example.org/onto/prop/google_developer_connect_connection_annotations">
    <rdfs:label>annotations</rdfs:label>
    <rdfs:comment>Optional. Allows clients to store small amounts of arbitrary data.

**Note**: This field is non-authoritative, and will only manage the annotations present in your configuration.
Please refer to the field 'effective_annotations' for all of the annotations present on the resource.</rdfs:comment>
    <rdfs:domain rdf:resource="http://example.org/onto/class/google_developer_connect_connection"/>
    <rdfs:range rdf:resource="http://www.w3.org/2001/XMLSchema#string"/>
  </owl:DatatypeProperty>
  <owl:DatatypeProperty rdf:about="http://example.org/onto/prop/google_developer_connect_connection_connection_id">
    <rdfs:label>connection_id</rdfs:label>
    <rdfs:comment>Required. Id of the requesting object
If auto-generating Id server-side, remove this field and
connection_id from the method_signature of Create RPC</rdfs:comment>
    <rdfs:domain rdf:resource="http://example.org/onto/class/google_developer_connect_connection"/>
    <rdfs:range rdf:resource="http://www.w3.org/2001/XMLSchema#string"/>
  </owl:DatatypeProperty>
  <owl:DatatypeProperty rdf:about="http://example.org/onto/prop/google_developer_connect_connection_create_time">
    <rdfs:label>create_time</rdfs:label>
    <rdfs:comment>Output only. [Output only] Create timestamp</rdfs:comment>
    <rdfs:domain rdf:resource="http://example.org/onto/class/google_developer_connect_connection"/>
    <rdfs:range rdf:resource="http://www.w3.org/2001/XMLSchema#string"/>
  </owl:DatatypeProperty>
  <owl:DatatypeProperty rdf:about="http://example.org/onto/prop/google_developer_connect_connection_delete_time">
    <rdfs:label>delete_time</rdfs:label>
    <rdfs:comment>Output only. [Output only] Delete timestamp</rdfs:comment>
    <rdfs:domain rdf:resource="http://example.org/onto/class/google_developer_connect_connection"/>
    <rdfs:range rdf:resource="http://www.w3.org/2001/XMLSchema#string"/>
  </owl:DatatypeProperty>
  <owl:DatatypeProperty rdf:about="http://example.org/onto/prop/google_developer_connect_connection_disabled">
    <rdfs:label>disabled</rdfs:label>
    <rdfs:comment>Optional. If disabled is set to true, functionality is disabled for this connection.
Repository based API methods and webhooks processing for repositories in
this connection will be disabled.</rdfs:comment>
    <rdfs:domain rdf:resource="http://example.org/onto/class/google_developer_connect_connection"/>
    <rdfs:range rdf:resource="http://www.w3.org/2001/XMLSchema#string"/>
  </owl:DatatypeProperty>
  <owl:DatatypeProperty rdf:about="http://example.org/onto/prop/google_developer_connect_connection_effective_annotations">
    <rdfs:label>effective_annotations</rdfs:label>
    <rdfs:comment>All of annotations (key/value pairs) present on the resource in GCP, including the annotations configured through Terraform, other clients and services.</rdfs:comment>
    <rdfs:domain rdf:resource="http://example.org/onto/class/google_developer_connect_connection"/>
    <rdfs:range rdf:resource="http://www.w3.org/2001/XMLSchema#string"/>
  </owl:DatatypeProperty>
  <owl:DatatypeProperty rdf:about="http://example.org/onto/prop/google_developer_connect_connection_effective_labels">
    <rdfs:label>effective_labels</rdfs:label>
    <rdfs:comment>All of labels (key/value pairs) present on the resource in GCP, including the labels configured through Terraform, other clients and services.</rdfs:comment>
    <rdfs:domain rdf:resource="http://example.org/onto/class/google_developer_connect_connection"/>
    <rdfs:range rdf:resource="http://www.w3.org/2001/XMLSchema#string"/>
  </owl:DatatypeProperty>
  <owl:DatatypeProperty rdf:about="http://example.org/onto/prop/google_developer_connect_connection_etag">
    <rdfs:label>etag</rdfs:label>
    <rdfs:comment>Optional. This checksum is computed by the server based on the value of other
fields, and may be sent on update and delete requests to ensure the
client has an up-to-date value before proceeding.</rdfs:comment>
    <rdfs:domain rdf:resource="http://example.org/onto/class/google_developer_connect_connection"/>
    <rdfs:range rdf:resource="http://www.w3.org/2001/XMLSchema#string"/>
  </owl:DatatypeProperty>
  <owl:DatatypeProperty rdf:about="http://example.org/onto/prop/google_developer_connect_connection_id">
    <rdfs:label>id</rdfs:label>
    <rdfs:domain rdf:resource="http://example.org/onto/class/google_developer_connect_connection"/>
    <rdfs:range rdf:resource="http://www.w3.org/2001/XMLSchema#string"/>
  </owl:DatatypeProperty>
  <owl:DatatypeProperty rdf:about="http://example.org/onto/prop/google_developer_connect_connection_installation_state">
    <rdfs:label>installation_state</rdfs:label>
    <rdfs:comment>Describes stage and necessary actions to be taken by the
user to complete the installation. Used for GitHub and GitHub Enterprise
based connections.</rdfs:comment>
    <rdfs:domain rdf:resource="http://example.org/onto/class/google_developer_connect_connection"/>
    <rdfs:range rdf:resource="http://www.w3.org/2001/XMLSchema#string"/>
  </owl:DatatypeProperty>
  <owl:DatatypeProperty rdf:about="http://example.org/onto/prop/google_developer_connect_connection_labels">
    <rdfs:label>labels</rdfs:label>
    <rdfs:comment>Optional. Labels as key value pairs

**Note**: This field is non-authoritative, and will only manage the labels present in your configuration.
Please refer to the field 'effective_labels' for all of the labels present on the resource.</rdfs:comment>
    <rdfs:domain rdf:resource="http://example.org/onto/class/google_developer_connect_connection"/>
    <rdfs:range rdf:resource="http://www.w3.org/2001/XMLSchema#string"/>
  </owl:DatatypeProperty>
  <owl:DatatypeProperty rdf:about="http://example.org/onto/prop/google_developer_connect_connection_location">
    <rdfs:label>location</rdfs:label>
    <rdfs:comment>Resource ID segment making up resource 'name'. It identifies the resource within its parent collection as described in https://google.aip.dev/122.</rdfs:comment>
    <rdfs:domain rdf:resource="http://example.org/onto/class/google_developer_connect_connection"/>
    <rdfs:range rdf:resource="http://www.w3.org/2001/XMLSchema#string"/>
  </owl:DatatypeProperty>
  <owl:DatatypeProperty rdf:about="http://example.org/onto/prop/google_developer_connect_connection_name">
    <rdfs:label>name</rdfs:label>
    <rdfs:comment>Identifier. The resource name of the connection, in the format
'projects/{project}/locations/{location}/connections/{connection_id}'.</rdfs:comment>
    <rdfs:domain rdf:resource="http://example.org/onto/class/google_developer_connect_connection"/>
    <rdfs:range rdf:resource="http://www.w3.org/2001/XMLSchema#string"/>
  </owl:DatatypeProperty>
  <owl:DatatypeProperty rdf:about="http://example.org/onto/prop/google_developer_connect_connection_project">
    <rdfs:label>project</rdfs:label>
    <rdfs:domain rdf:resource="http://example.org/onto/class/google_developer_connect_connection"/>
    <rdfs:range rdf:resource="http://www.w3.org/2001/XMLSchema#string"/>
  </owl:DatatypeProperty>
  <owl:DatatypeProperty rdf:about="http://example.org/onto/prop/google_developer_connect_connection_reconciling">
    <rdfs:label>reconciling</rdfs:label>
    <rdfs:comment>Output only. Set to true when the connection is being set up or updated in the
background.</rdfs:comment>
    <rdfs:domain rdf:resource="http://example.org/onto/class/google_developer_connect_connection"/>
    <rdfs:range rdf:resource="http://www.w3.org/2001/XMLSchema#string"/>
  </owl:DatatypeProperty>
  <owl:DatatypeProperty rdf:about="http://example.org/onto/prop/google_developer_connect_connection_terraform_labels">
    <rdfs:label>terraform_labels</rdfs:label>
    <rdfs:comment>The combination of labels configured directly on the resource
 and default labels configured on the provider.</rdfs:comment>
    <rdfs:domain rdf:resource="http://example.org/onto/class/google_developer_connect_connection"/>
    <rdfs:range rdf:resource="http://www.w3.org/2001/XMLSchema#string"/>
  </owl:DatatypeProperty>
  <owl:DatatypeProperty rdf:about="http://example.org/onto/prop/google_developer_connect_connection_uid">
    <rdfs:label>uid</rdfs:label>
    <rdfs:comment>Output only. A system-assigned unique identifier for a the GitRepositoryLink.</rdfs:comment>
    <rdfs:domain rdf:resource="http://example.org/onto/class/google_developer_connect_connection"/>
    <rdfs:range rdf:resource="http://www.w3.org/2001/XMLSchema#string"/>
  </owl:DatatypeProperty>
  <owl:DatatypeProperty rdf:about="http://example.org/onto/prop/google_developer_connect_connection_update_time">
    <rdfs:label>update_time</rdfs:label>
    <rdfs:comment>Output only. [Output only] Update timestamp</rdfs:comment>
    <rdfs:domain rdf:resource="http://example.org/onto/class/google_developer_connect_connection"/>
    <rdfs:range rdf:resource="http://www.w3.org/2001/XMLSchema#string"/>
  </owl:DatatypeProperty>
  <owl:DatatypeProperty rdf:about="http://example.org/onto/prop/google_developer_connect_connection_webhook_secret_secret_version">
    <rdfs:label>webhook_secret_secret_version</rdfs:label>
    <rdfs:comment>Required. Immutable. SecretManager resource containing the webhook secret used to verify webhook
events, formatted as 'projects/*/secrets/*/versions/*'. This is used to
validate and create webhooks.</rdfs:comment>
    <rdfs:domain rdf:resource="http://example.org/onto/class/google_developer_connect_connection"/>
    <rdfs:range rdf:resource="http://www.w3.org/2001/XMLSchema#string"/>
  </owl:DatatypeProperty>
  <owl:DatatypeProperty rdf:about="http://example.org/onto/prop/google_developer_connect_connection_workspace">
    <rdfs:label>workspace</rdfs:label>
    <rdfs:comment>Required. The Bitbucket Cloud Workspace ID to be connected to Google Cloud Platform.</rdfs:comment>
    <rdfs:domain rdf:resource="http://example.org/onto/class/google_developer_connect_connection"/>
    <rdfs:range rdf:resource="http://www.w3.org/2001/XMLSchema#string"/>
  </owl:DatatypeProperty>
  <owl:DatatypeProperty rdf:about="http://example.org/onto/prop/google_developer_connect_connection_user_token_secret_version">
    <rdfs:label>user_token_secret_version</rdfs:label>
    <rdfs:comment>Required. A SecretManager resource containing the user token that authorizes
the Developer Connect connection. Format:
'projects/*/secrets/*/versions/*'.</rdfs:comment>
    <rdfs:domain rdf:resource="http://example.org/onto/class/google_developer_connect_connection"/>
    <rdfs:range rdf:resource="http://www.w3.org/2001/XMLSchema#string"/>
  </owl:DatatypeProperty>
  <owl:DatatypeProperty rdf:about="http://example.org/onto/prop/google_developer_connect_connection_username">
    <rdfs:label>username</rdfs:label>
    <rdfs:comment>Output only. The username associated with this token.</rdfs:comment>
    <rdfs:domain rdf:resource="http://example.org/onto/class/google_developer_connect_connection"/>
    <rdfs:range rdf:resource="http://www.w3.org/2001/XMLSchema#string"/>
  </owl:DatatypeProperty>
  <owl:DatatypeProperty rdf:about="http://example.org/onto/prop/google_developer_connect_connection_user_token_secret_version">
    <rdfs:label>user_token_secret_version</rdfs:label>
    <rdfs:comment>Required. A SecretManager resource containing the user token that authorizes
the Developer Connect connection. Format:
'projects/*/secrets/*/versions/*'.</rdfs:comment>
    <rdfs:domain rdf:resource="http://example.org/onto/class/google_developer_connect_connection"/>
    <rdfs:range rdf:resource="http://www.w3.org/2001/XMLSchema#string"/>
  </owl:DatatypeProperty>
  <owl:DatatypeProperty rdf:about="http://example.org/onto/prop/google_developer_connect_connection_username">
    <rdfs:label>username</rdfs:label>
    <rdfs:comment>Output only. The username associated with this token.</rdfs:comment>
    <rdfs:domain rdf:resource="http://example.org/onto/class/google_developer_connect_connection"/>
    <rdfs:range rdf:resource="http://www.w3.org/2001/XMLSchema#string"/>
  </owl:DatatypeProperty>
  <owl:DatatypeProperty rdf:about="http://example.org/onto/prop/google_developer_connect_connection_host_uri">
    <rdfs:label>host_uri</rdfs:label>
    <rdfs:comment>Required. The URI of the Bitbucket Data Center host this connection is for.</rdfs:comment>
    <rdfs:domain rdf:resource="http://example.org/onto/class/google_developer_connect_connection"/>
    <rdfs:range rdf:resource="http://www.w3.org/2001/XMLSchema#string"/>
  </owl:DatatypeProperty>
  <owl:DatatypeProperty rdf:about="http://example.org/onto/prop/google_developer_connect_connection_server_version">
    <rdfs:label>server_version</rdfs:label>
    <rdfs:comment>Output only. Version of the Bitbucket Data Center server running on the 'host_uri'.</rdfs:comment>
    <rdfs:domain rdf:resource="http://example.org/onto/class/google_developer_connect_connection"/>
    <rdfs:range rdf:resource="http://www.w3.org/2001/XMLSchema#string"/>
  </owl:DatatypeProperty>
  <owl:DatatypeProperty rdf:about="http://example.org/onto/prop/google_developer_connect_connection_ssl_ca_certificate">
    <rdfs:label>ssl_ca_certificate</rdfs:label>
    <rdfs:comment>Optional. SSL certificate authority to trust when making requests to Bitbucket Data
Center.</rdfs:comment>
    <rdfs:domain rdf:resource="http://example.org/onto/class/google_developer_connect_connection"/>
    <rdfs:range rdf:resource="http://www.w3.org/2001/XMLSchema#string"/>
  </owl:DatatypeProperty>
  <owl:DatatypeProperty rdf:about="http://example.org/onto/prop/google_developer_connect_connection_webhook_secret_secret_version">
    <rdfs:label>webhook_secret_secret_version</rdfs:label>
    <rdfs:comment>Required. Immutable. SecretManager resource containing the webhook secret used to verify webhook
events, formatted as 'projects/*/secrets/*/versions/*'. This is used to
validate webhooks.</rdfs:comment>
    <rdfs:domain rdf:resource="http://example.org/onto/class/google_developer_connect_connection"/>
    <rdfs:range rdf:resource="http://www.w3.org/2001/XMLSchema#string"/>
  </owl:DatatypeProperty>
  <owl:DatatypeProperty rdf:about="http://example.org/onto/prop/google_developer_connect_connection_user_token_secret_version">
    <rdfs:label>user_token_secret_version</rdfs:label>
    <rdfs:comment>Required. A SecretManager resource containing the user token that authorizes
the Developer Connect connection. Format:
'projects/*/secrets/*/versions/*'.</rdfs:comment>
    <rdfs:domain rdf:resource="http://example.org/onto/class/google_developer_connect_connection"/>
    <rdfs:range rdf:resource="http://www.w3.org/2001/XMLSchema#string"/>
  </owl:DatatypeProperty>
  <owl:DatatypeProperty rdf:about="http://example.org/onto/prop/google_developer_connect_connection_username">
    <rdfs:label>username</rdfs:label>
    <rdfs:comment>Output only. The username associated with this token.</rdfs:comment>
    <rdfs:domain rdf:resource="http://example.org/onto/class/google_developer_connect_connection"/>
    <rdfs:range rdf:resource="http://www.w3.org/2001/XMLSchema#string"/>
  </owl:DatatypeProperty>
  <owl:DatatypeProperty rdf:about="http://example.org/onto/prop/google_developer_connect_connection_user_token_secret_version">
    <rdfs:label>user_token_secret_version</rdfs:label>
    <rdfs:comment>Required. A SecretManager resource containing the user token that authorizes
the Developer Connect connection. Format:
'projects/*/secrets/*/versions/*'.</rdfs:comment>
    <rdfs:domain rdf:resource="http://example.org/onto/class/google_developer_connect_connection"/>
    <rdfs:range rdf:resource="http://www.w3.org/2001/XMLSchema#string"/>
  </owl:DatatypeProperty>
  <owl:DatatypeProperty rdf:about="http://example.org/onto/prop/google_developer_connect_connection_username">
    <rdfs:label>username</rdfs:label>
    <rdfs:comment>Output only. The username associated with this token.</rdfs:comment>
    <rdfs:domain rdf:resource="http://example.org/onto/class/google_developer_connect_connection"/>
    <rdfs:range rdf:resource="http://www.w3.org/2001/XMLSchema#string"/>
  </owl:DatatypeProperty>
  <owl:DatatypeProperty rdf:about="http://example.org/onto/prop/google_developer_connect_connection_service">
    <rdfs:label>service</rdfs:label>
    <rdfs:comment>Required. The Service Directory service name.
Format:
projects/{project}/locations/{location}/namespaces/{namespace}/services/{service}.</rdfs:comment>
    <rdfs:domain rdf:resource="http://example.org/onto/class/google_developer_connect_connection"/>
    <rdfs:range rdf:resource="http://www.w3.org/2001/XMLSchema#string"/>
  </owl:DatatypeProperty>
  <owl:DatatypeProperty rdf:about="http://example.org/onto/prop/google_developer_connect_connection_key_reference">
    <rdfs:label>key_reference</rdfs:label>
    <rdfs:comment>Required. The name of the key which is used to encrypt/decrypt customer data. For key
in Cloud KMS, the key should be in the format of
'projects/*/locations/*/keyRings/*/cryptoKeys/*'.</rdfs:comment>
    <rdfs:domain rdf:resource="http://example.org/onto/class/google_developer_connect_connection"/>
    <rdfs:range rdf:resource="http://www.w3.org/2001/XMLSchema#string"/>
  </owl:DatatypeProperty>
  <owl:DatatypeProperty rdf:about="http://example.org/onto/prop/google_developer_connect_connection_app_installation_id">
    <rdfs:label>app_installation_id</rdfs:label>
    <rdfs:comment>Optional. GitHub App installation id.</rdfs:comment>
    <rdfs:domain rdf:resource="http://example.org/onto/class/google_developer_connect_connection"/>
    <rdfs:range rdf:resource="http://www.w3.org/2001/XMLSchema#string"/>
  </owl:DatatypeProperty>
  <owl:DatatypeProperty rdf:about="http://example.org/onto/prop/google_developer_connect_connection_github_app">
    <rdfs:label>github_app</rdfs:label>
    <rdfs:comment>Required. Immutable. The GitHub Application that was installed to the GitHub user or
organization.
Possible values:
GIT_HUB_APP_UNSPECIFIED
DEVELOPER_CONNECT
FIREBASE</rdfs:comment>
    <rdfs:domain rdf:resource="http://example.org/onto/class/google_developer_connect_connection"/>
    <rdfs:range rdf:resource="http://www.w3.org/2001/XMLSchema#string"/>
  </owl:DatatypeProperty>
  <owl:DatatypeProperty rdf:about="http://example.org/onto/prop/google_developer_connect_connection_installation_uri">
    <rdfs:label>installation_uri</rdfs:label>
    <rdfs:comment>Output only. The URI to navigate to in order to manage the installation associated
with this GitHubConfig.</rdfs:comment>
    <rdfs:domain rdf:resource="http://example.org/onto/class/google_developer_connect_connection"/>
    <rdfs:range rdf:resource="http://www.w3.org/2001/XMLSchema#string"/>
  </owl:DatatypeProperty>
  <owl:DatatypeProperty rdf:about="http://example.org/onto/prop/google_developer_connect_connection_oauth_token_secret_version">
    <rdfs:label>oauth_token_secret_version</rdfs:label>
    <rdfs:comment>Required. A SecretManager resource containing the OAuth token that authorizes
the connection. Format: 'projects/*/secrets/*/versions/*'.</rdfs:comment>
    <rdfs:domain rdf:resource="http://example.org/onto/class/google_developer_connect_connection"/>
    <rdfs:range rdf:resource="http://www.w3.org/2001/XMLSchema#string"/>
  </owl:DatatypeProperty>
  <owl:DatatypeProperty rdf:about="http://example.org/onto/prop/google_developer_connect_connection_username">
    <rdfs:label>username</rdfs:label>
    <rdfs:comment>Output only. The username associated with this token.</rdfs:comment>
    <rdfs:domain rdf:resource="http://example.org/onto/class/google_developer_connect_connection"/>
    <rdfs:range rdf:resource="http://www.w3.org/2001/XMLSchema#string"/>
  </owl:DatatypeProperty>
  <owl:DatatypeProperty rdf:about="http://example.org/onto/prop/google_developer_connect_connection_app_id">
    <rdfs:label>app_id</rdfs:label>
    <rdfs:comment>Optional. ID of the GitHub App created from the manifest.</rdfs:comment>
    <rdfs:domain rdf:resource="http://example.org/onto/class/google_developer_connect_connection"/>
    <rdfs:range rdf:resource="http://www.w3.org/2001/XMLSchema#string"/>
  </owl:DatatypeProperty>
  <owl:DatatypeProperty rdf:about="http://example.org/onto/prop/google_developer_connect_connection_app_installation_id">
    <rdfs:label>app_installation_id</rdfs:label>
    <rdfs:comment>Optional. ID of the installation of the GitHub App.</rdfs:comment>
    <rdfs:domain rdf:resource="http://example.org/onto/class/google_developer_connect_connection"/>
    <rdfs:range rdf:resource="http://www.w3.org/2001/XMLSchema#string"/>
  </owl:DatatypeProperty>
  <owl:DatatypeProperty rdf:about="http://example.org/onto/prop/google_developer_connect_connection_app_slug">
    <rdfs:label>app_slug</rdfs:label>
    <rdfs:comment>Output only. The URL-friendly name of the GitHub App.</rdfs:comment>
    <rdfs:domain rdf:resource="http://example.org/onto/class/google_developer_connect_connection"/>
    <rdfs:range rdf:resource="http://www.w3.org/2001/XMLSchema#string"/>
  </owl:DatatypeProperty>
  <owl:DatatypeProperty rdf:about="http://example.org/onto/prop/google_developer_connect_connection_host_uri">
    <rdfs:label>host_uri</rdfs:label>
    <rdfs:comment>Required. The URI of the GitHub Enterprise host this connection is for.</rdfs:comment>
    <rdfs:domain rdf:resource="http://example.org/onto/class/google_developer_connect_connection"/>
    <rdfs:range rdf:resource="http://www.w3.org/2001/XMLSchema#string"/>
  </owl:DatatypeProperty>
  <owl:DatatypeProperty rdf:about="http://example.org/onto/prop/google_developer_connect_connection_installation_uri">
    <rdfs:label>installation_uri</rdfs:label>
    <rdfs:comment>Output only. The URI to navigate to in order to manage the installation associated
with this GitHubEnterpriseConfig.</rdfs:comment>
    <rdfs:domain rdf:resource="http://example.org/onto/class/google_developer_connect_connection"/>
    <rdfs:range rdf:resource="http://www.w3.org/2001/XMLSchema#string"/>
  </owl:DatatypeProperty>
  <owl:DatatypeProperty rdf:about="http://example.org/onto/prop/google_developer_connect_connection_private_key_secret_version">
    <rdfs:label>private_key_secret_version</rdfs:label>
    <rdfs:comment>Optional. SecretManager resource containing the private key of the GitHub App,
formatted as 'projects/*/secrets/*/versions/*'.</rdfs:comment>
    <rdfs:domain rdf:resource="http://example.org/onto/class/google_developer_connect_connection"/>
    <rdfs:range rdf:resource="http://www.w3.org/2001/XMLSchema#string"/>
  </owl:DatatypeProperty>
  <owl:DatatypeProperty rdf:about="http://example.org/onto/prop/google_developer_connect_connection_server_version">
    <rdfs:label>server_version</rdfs:label>
    <rdfs:comment>Output only. GitHub Enterprise version installed at the host_uri.</rdfs:comment>
    <rdfs:domain rdf:resource="http://example.org/onto/class/google_developer_connect_connection"/>
    <rdfs:range rdf:resource="http://www.w3.org/2001/XMLSchema#string"/>
  </owl:DatatypeProperty>
  <owl:DatatypeProperty rdf:about="http://example.org/onto/prop/google_developer_connect_connection_ssl_ca_certificate">
    <rdfs:label>ssl_ca_certificate</rdfs:label>
    <rdfs:comment>Optional. SSL certificate to use for requests to GitHub Enterprise.</rdfs:comment>
    <rdfs:domain rdf:resource="http://example.org/onto/class/google_developer_connect_connection"/>
    <rdfs:range rdf:resource="http://www.w3.org/2001/XMLSchema#string"/>
  </owl:DatatypeProperty>
  <owl:DatatypeProperty rdf:about="http://example.org/onto/prop/google_developer_connect_connection_webhook_secret_secret_version">
    <rdfs:label>webhook_secret_secret_version</rdfs:label>
    <rdfs:comment>Optional. SecretManager resource containing the webhook secret of the GitHub App,
formatted as 'projects/*/secrets/*/versions/*'.</rdfs:comment>
    <rdfs:domain rdf:resource="http://example.org/onto/class/google_developer_connect_connection"/>
    <rdfs:range rdf:resource="http://www.w3.org/2001/XMLSchema#string"/>
  </owl:DatatypeProperty>
  <owl:DatatypeProperty rdf:about="http://example.org/onto/prop/google_developer_connect_connection_service">
    <rdfs:label>service</rdfs:label>
    <rdfs:comment>Required. The Service Directory service name.
Format:
projects/{project}/locations/{location}/namespaces/{namespace}/services/{service}.</rdfs:comment>
    <rdfs:domain rdf:resource="http://example.org/onto/class/google_developer_connect_connection"/>
    <rdfs:range rdf:resource="http://www.w3.org/2001/XMLSchema#string"/>
  </owl:DatatypeProperty>
  <owl:DatatypeProperty rdf:about="http://example.org/onto/prop/google_developer_connect_connection_webhook_secret_secret_version">
    <rdfs:label>webhook_secret_secret_version</rdfs:label>
    <rdfs:comment>Required. Immutable. SecretManager resource containing the webhook secret of a GitLab project,
formatted as 'projects/*/secrets/*/versions/*'. This is used to validate
webhooks.</rdfs:comment>
    <rdfs:domain rdf:resource="http://example.org/onto/class/google_developer_connect_connection"/>
    <rdfs:range rdf:resource="http://www.w3.org/2001/XMLSchema#string"/>
  </owl:DatatypeProperty>
  <owl:DatatypeProperty rdf:about="http://example.org/onto/prop/google_developer_connect_connection_user_token_secret_version">
    <rdfs:label>user_token_secret_version</rdfs:label>
    <rdfs:comment>Required. A SecretManager resource containing the user token that authorizes
the Developer Connect connection. Format:
'projects/*/secrets/*/versions/*'.</rdfs:comment>
    <rdfs:domain rdf:resource="http://example.org/onto/class/google_developer_connect_connection"/>
    <rdfs:range rdf:resource="http://www.w3.org/2001/XMLSchema#string"/>
  </owl:DatatypeProperty>
  <owl:DatatypeProperty rdf:about="http://example.org/onto/prop/google_developer_connect_connection_username">
    <rdfs:label>username</rdfs:label>
    <rdfs:comment>Output only. The username associated with this token.</rdfs:comment>
    <rdfs:domain rdf:resource="http://example.org/onto/class/google_developer_connect_connection"/>
    <rdfs:range rdf:resource="http://www.w3.org/2001/XMLSchema#string"/>
  </owl:DatatypeProperty>
  <owl:DatatypeProperty rdf:about="http://example.org/onto/prop/google_developer_connect_connection_user_token_secret_version">
    <rdfs:label>user_token_secret_version</rdfs:label>
    <rdfs:comment>Required. A SecretManager resource containing the user token that authorizes
the Developer Connect connection. Format:
'projects/*/secrets/*/versions/*'.</rdfs:comment>
    <rdfs:domain rdf:resource="http://example.org/onto/class/google_developer_connect_connection"/>
    <rdfs:range rdf:resource="http://www.w3.org/2001/XMLSchema#string"/>
  </owl:DatatypeProperty>
  <owl:DatatypeProperty rdf:about="http://example.org/onto/prop/google_developer_connect_connection_username">
    <rdfs:label>username</rdfs:label>
    <rdfs:comment>Output only. The username associated with this token.</rdfs:comment>
    <rdfs:domain rdf:resource="http://example.org/onto/class/google_developer_connect_connection"/>
    <rdfs:range rdf:resource="http://www.w3.org/2001/XMLSchema#string"/>
  </owl:DatatypeProperty>
  <owl:DatatypeProperty rdf:about="http://example.org/onto/prop/google_developer_connect_connection_host_uri">
    <rdfs:label>host_uri</rdfs:label>
    <rdfs:comment>Required. The URI of the GitLab Enterprise host this connection is for.</rdfs:comment>
    <rdfs:domain rdf:resource="http://example.org/onto/class/google_developer_connect_connection"/>
    <rdfs:range rdf:resource="http://www.w3.org/2001/XMLSchema#string"/>
  </owl:DatatypeProperty>
  <owl:DatatypeProperty rdf:about="http://example.org/onto/prop/google_developer_connect_connection_server_version">
    <rdfs:label>server_version</rdfs:label>
    <rdfs:comment>Output only. Version of the GitLab Enterprise server running on the 'host_uri'.</rdfs:comment>
    <rdfs:domain rdf:resource="http://example.org/onto/class/google_developer_connect_connection"/>
    <rdfs:range rdf:resource="http://www.w3.org/2001/XMLSchema#string"/>
  </owl:DatatypeProperty>
  <owl:DatatypeProperty rdf:about="http://example.org/onto/prop/google_developer_connect_connection_ssl_ca_certificate">
    <rdfs:label>ssl_ca_certificate</rdfs:label>
    <rdfs:comment>Optional. SSL Certificate Authority certificate to use for requests to GitLab
Enterprise instance.</rdfs:comment>
    <rdfs:domain rdf:resource="http://example.org/onto/class/google_developer_connect_connection"/>
    <rdfs:range rdf:resource="http://www.w3.org/2001/XMLSchema#string"/>
  </owl:DatatypeProperty>
  <owl:DatatypeProperty rdf:about="http://example.org/onto/prop/google_developer_connect_connection_webhook_secret_secret_version">
    <rdfs:label>webhook_secret_secret_version</rdfs:label>
    <rdfs:comment>Required. Immutable. SecretManager resource containing the webhook secret of a GitLab project,
formatted as 'projects/*/secrets/*/versions/*'. This is used to validate
webhooks.</rdfs:comment>
    <rdfs:domain rdf:resource="http://example.org/onto/class/google_developer_connect_connection"/>
    <rdfs:range rdf:resource="http://www.w3.org/2001/XMLSchema#string"/>
  </owl:DatatypeProperty>
  <owl:DatatypeProperty rdf:about="http://example.org/onto/prop/google_developer_connect_connection_user_token_secret_version">
    <rdfs:label>user_token_secret_version</rdfs:label>
    <rdfs:comment>Required. A SecretManager resource containing the user token that authorizes
the Developer Connect connection. Format:
'projects/*/secrets/*/versions/*'.</rdfs:comment>
    <rdfs:domain rdf:resource="http://example.org/onto/class/google_developer_connect_connection"/>
    <rdfs:range rdf:resource="http://www.w3.org/2001/XMLSchema#string"/>
  </owl:DatatypeProperty>
  <owl:DatatypeProperty rdf:about="http://example.org/onto/prop/google_developer_connect_connection_username">
    <rdfs:label>username</rdfs:label>
    <rdfs:comment>Output only. The username associated with this token.</rdfs:comment>
    <rdfs:domain rdf:resource="http://example.org/onto/class/google_developer_connect_connection"/>
    <rdfs:range rdf:resource="http://www.w3.org/2001/XMLSchema#string"/>
  </owl:DatatypeProperty>
  <owl:DatatypeProperty rdf:about="http://example.org/onto/prop/google_developer_connect_connection_user_token_secret_version">
    <rdfs:label>user_token_secret_version</rdfs:label>
    <rdfs:comment>Required. A SecretManager resource containing the user token that authorizes
the Developer Connect connection. Format:
'projects/*/secrets/*/versions/*'.</rdfs:comment>
    <rdfs:domain rdf:resource="http://example.org/onto/class/google_developer_connect_connection"/>
    <rdfs:range rdf:resource="http://www.w3.org/2001/XMLSchema#string"/>
  </owl:DatatypeProperty>
  <owl:DatatypeProperty rdf:about="http://example.org/onto/prop/google_developer_connect_connection_username">
    <rdfs:label>username</rdfs:label>
    <rdfs:comment>Output only. The username associated with this token.</rdfs:comment>
    <rdfs:domain rdf:resource="http://example.org/onto/class/google_developer_connect_connection"/>
    <rdfs:range rdf:resource="http://www.w3.org/2001/XMLSchema#string"/>
  </owl:DatatypeProperty>
  <owl:DatatypeProperty rdf:about="http://example.org/onto/prop/google_developer_connect_connection_service">
    <rdfs:label>service</rdfs:label>
    <rdfs:comment>Required. The Service Directory service name.
Format:
projects/{project}/locations/{location}/namespaces/{namespace}/services/{service}.</rdfs:comment>
    <rdfs:domain rdf:resource="http://example.org/onto/class/google_developer_connect_connection"/>
    <rdfs:range rdf:resource="http://www.w3.org/2001/XMLSchema#string"/>
  </owl:DatatypeProperty>
  <owl:DatatypeProperty rdf:about="http://example.org/onto/prop/google_developer_connect_connection_create">
    <rdfs:label>create</rdfs:label>
    <rdfs:domain rdf:resource="http://example.org/onto/class/google_developer_connect_connection"/>
    <rdfs:range rdf:resource="http://www.w3.org/2001/XMLSchema#string"/>
  </owl:DatatypeProperty>
  <owl:DatatypeProperty rdf:about="http://example.org/onto/prop/google_developer_connect_connection_delete">
    <rdfs:label>delete</rdfs:label>
    <rdfs:domain rdf:resource="http://example.org/onto/class/google_developer_connect_connection"/>
    <rdfs:range rdf:resource="http://www.w3.org/2001/XMLSchema#string"/>
  </owl:DatatypeProperty>
  <owl:DatatypeProperty rdf:about="http://example.org/onto/prop/google_developer_connect_connection_update">
    <rdfs:label>update</rdfs:label>
    <rdfs:domain rdf:resource="http://example.org/onto/class/google_developer_connect_connection"/>
    <rdfs:range rdf:resource="http://www.w3.org/2001/XMLSchema#string"/>
  </owl:DatatypeProperty>
</rdf:RDF>
