<?xml version="1.0" encoding="UTF-8"?>
<rdf:RDF
  xmlns:rdf="http://www.w3.org/1999/02/22-rdf-syntax-ns#"
  xmlns:rdfs="http://www.w3.org/2000/01/rdf-schema#"
  xmlns:owl="http://www.w3.org/2002/07/owl#"
  xmlns:xsd="http://www.w3.org/2001/XMLSchema#"
  xml:base="http://example.org/onto/">
  <owl:Class rdf:about="http://example.org/onto/class/google_spanner_backup_schedule">
    <rdfs:label>google_spanner_backup_schedule</rdfs:label>
    <rdfs:comment>#
#     ***     AUTO GENERATED CODE    ***    Type: MMv1     ***
#
# ----------------------------------------------------------------------------
#
#     This code is generated by Magic Modules using the following:
#
#     Configuration: https:#github.com/GoogleCloudPlatform/magic-modules/tree/main/mmv1/products/spanner/BackupSchedule.yaml
#     Template:      https:#github.com/GoogleCloudPlatform/magic-modules/tree/main/mmv1/templates/terraform/resource.html.markdown.tmpl
#
#     DO NOT EDIT this file directly. Any changes made to this file will be
#     overwritten during the next generation cycle.
#
# ----------------------------------------------------------------------------
subcategory: "Cloud Spanner"
description: |-
  A backup schedule for a Cloud Spanner Database.
---</rdfs:comment>
  </owl:Class>
  <owl:DatatypeProperty rdf:about="http://example.org/onto/prop/google_spanner_backup_schedule_database">
    <rdfs:label>database</rdfs:label>
    <rdfs:comment>The database to create the backup schedule on.</rdfs:comment>
    <rdfs:domain rdf:resource="http://example.org/onto/class/google_spanner_backup_schedule"/>
    <rdfs:range rdf:resource="http://www.w3.org/2001/XMLSchema#string"/>
  </owl:DatatypeProperty>
  <owl:DatatypeProperty rdf:about="http://example.org/onto/prop/google_spanner_backup_schedule_id">
    <rdfs:label>id</rdfs:label>
    <rdfs:domain rdf:resource="http://example.org/onto/class/google_spanner_backup_schedule"/>
    <rdfs:range rdf:resource="http://www.w3.org/2001/XMLSchema#string"/>
  </owl:DatatypeProperty>
  <owl:DatatypeProperty rdf:about="http://example.org/onto/prop/google_spanner_backup_schedule_instance">
    <rdfs:label>instance</rdfs:label>
    <rdfs:comment>The instance to create the database on.</rdfs:comment>
    <rdfs:domain rdf:resource="http://example.org/onto/class/google_spanner_backup_schedule"/>
    <rdfs:range rdf:resource="http://www.w3.org/2001/XMLSchema#string"/>
  </owl:DatatypeProperty>
  <owl:DatatypeProperty rdf:about="http://example.org/onto/prop/google_spanner_backup_schedule_name">
    <rdfs:label>name</rdfs:label>
    <rdfs:comment>A unique identifier for the backup schedule, which cannot be changed after
the backup schedule is created. Values are of the form [a-z][-a-z0-9]*[a-z0-9].</rdfs:comment>
    <rdfs:domain rdf:resource="http://example.org/onto/class/google_spanner_backup_schedule"/>
    <rdfs:range rdf:resource="http://www.w3.org/2001/XMLSchema#string"/>
  </owl:DatatypeProperty>
  <owl:DatatypeProperty rdf:about="http://example.org/onto/prop/google_spanner_backup_schedule_project">
    <rdfs:label>project</rdfs:label>
    <rdfs:domain rdf:resource="http://example.org/onto/class/google_spanner_backup_schedule"/>
    <rdfs:range rdf:resource="http://www.w3.org/2001/XMLSchema#string"/>
  </owl:DatatypeProperty>
  <owl:DatatypeProperty rdf:about="http://example.org/onto/prop/google_spanner_backup_schedule_retention_duration">
    <rdfs:label>retention_duration</rdfs:label>
    <rdfs:comment>At what relative time in the future, compared to its creation time, the backup should be deleted, e.g. keep backups for 7 days.
A duration in seconds with up to nine fractional digits, ending with 's'. Example: '3.5s'.
You can set this to a value up to 366 days.</rdfs:comment>
    <rdfs:domain rdf:resource="http://example.org/onto/class/google_spanner_backup_schedule"/>
    <rdfs:range rdf:resource="http://www.w3.org/2001/XMLSchema#string"/>
  </owl:DatatypeProperty>
  <owl:DatatypeProperty rdf:about="http://example.org/onto/prop/google_spanner_backup_schedule_encryption_type">
    <rdfs:label>encryption_type</rdfs:label>
    <rdfs:comment>The encryption type of backups created by the backup schedule.
Possible values are USE_DATABASE_ENCRYPTION, GOOGLE_DEFAULT_ENCRYPTION, or CUSTOMER_MANAGED_ENCRYPTION.
If you use CUSTOMER_MANAGED_ENCRYPTION, you must specify a kmsKeyName.
If your backup type is incremental-backup, the encryption type must be GOOGLE_DEFAULT_ENCRYPTION. Possible values: ["USE_DATABASE_ENCRYPTION", "GOOGLE_DEFAULT_ENCRYPTION", "CUSTOMER_MANAGED_ENCRYPTION"]</rdfs:comment>
    <rdfs:domain rdf:resource="http://example.org/onto/class/google_spanner_backup_schedule"/>
    <rdfs:range rdf:resource="http://www.w3.org/2001/XMLSchema#string"/>
  </owl:DatatypeProperty>
  <owl:DatatypeProperty rdf:about="http://example.org/onto/prop/google_spanner_backup_schedule_kms_key_name">
    <rdfs:label>kms_key_name</rdfs:label>
    <rdfs:comment>The resource name of the Cloud KMS key to use for encryption.
Format: 'projects/{project}/locations/{location}/keyRings/{keyRing}/cryptoKeys/{cryptoKey}'</rdfs:comment>
    <rdfs:domain rdf:resource="http://example.org/onto/class/google_spanner_backup_schedule"/>
    <rdfs:range rdf:resource="http://www.w3.org/2001/XMLSchema#string"/>
  </owl:DatatypeProperty>
  <owl:DatatypeProperty rdf:about="http://example.org/onto/prop/google_spanner_backup_schedule_kms_key_names">
    <rdfs:label>kms_key_names</rdfs:label>
    <rdfs:comment>Fully qualified name of the KMS keys to use to encrypt this database. The keys must exist
in the same locations as the Spanner Database.</rdfs:comment>
    <rdfs:domain rdf:resource="http://example.org/onto/class/google_spanner_backup_schedule"/>
    <rdfs:range rdf:resource="http://www.w3.org/2001/XMLSchema#string"/>
  </owl:DatatypeProperty>
  <owl:DatatypeProperty rdf:about="http://example.org/onto/prop/google_spanner_backup_schedule_text">
    <rdfs:label>text</rdfs:label>
    <rdfs:comment>Textual representation of the crontab. User can customize the
backup frequency and the backup version time using the cron
expression. The version time must be in UTC timzeone.
The backup will contain an externally consistent copy of the
database at the version time. Allowed frequencies are 12 hour, 1 day,
1 week and 1 month. Examples of valid cron specifications:
  0 2/12 * * * : every 12 hours at (2, 14) hours past midnight in UTC.
  0 2,14 * * * : every 12 hours at (2,14) hours past midnight in UTC.
  0 2 * * *    : once a day at 2 past midnight in UTC.
  0 2 * * 0    : once a week every Sunday at 2 past midnight in UTC.
  0 2 8 * *    : once a month on 8th day at 2 past midnight in UTC.</rdfs:comment>
    <rdfs:domain rdf:resource="http://example.org/onto/class/google_spanner_backup_schedule"/>
    <rdfs:range rdf:resource="http://www.w3.org/2001/XMLSchema#string"/>
  </owl:DatatypeProperty>
  <owl:DatatypeProperty rdf:about="http://example.org/onto/prop/google_spanner_backup_schedule_create">
    <rdfs:label>create</rdfs:label>
    <rdfs:domain rdf:resource="http://example.org/onto/class/google_spanner_backup_schedule"/>
    <rdfs:range rdf:resource="http://www.w3.org/2001/XMLSchema#string"/>
  </owl:DatatypeProperty>
  <owl:DatatypeProperty rdf:about="http://example.org/onto/prop/google_spanner_backup_schedule_delete">
    <rdfs:label>delete</rdfs:label>
    <rdfs:domain rdf:resource="http://example.org/onto/class/google_spanner_backup_schedule"/>
    <rdfs:range rdf:resource="http://www.w3.org/2001/XMLSchema#string"/>
  </owl:DatatypeProperty>
  <owl:DatatypeProperty rdf:about="http://example.org/onto/prop/google_spanner_backup_schedule_update">
    <rdfs:label>update</rdfs:label>
    <rdfs:domain rdf:resource="http://example.org/onto/class/google_spanner_backup_schedule"/>
    <rdfs:range rdf:resource="http://www.w3.org/2001/XMLSchema#string"/>
  </owl:DatatypeProperty>
</rdf:RDF>
