<?xml version="1.0" encoding="UTF-8"?>
<rdf:RDF
  xmlns:rdf="http://www.w3.org/1999/02/22-rdf-syntax-ns#"
  xmlns:rdfs="http://www.w3.org/2000/01/rdf-schema#"
  xmlns:owl="http://www.w3.org/2002/07/owl#"
  xmlns:xsd="http://www.w3.org/2001/XMLSchema#"
  xml:base="http://example.org/onto/">
  <owl:Class rdf:about="http://example.org/onto/class/google_certificate_manager_trust_config">
    <rdfs:label>google_certificate_manager_trust_config</rdfs:label>
    <rdfs:comment>#
#     ***     AUTO GENERATED CODE    ***    Type: MMv1     ***
#
# ----------------------------------------------------------------------------
#
#     This code is generated by Magic Modules using the following:
#
#     Configuration: https:#github.com/GoogleCloudPlatform/magic-modules/tree/main/mmv1/products/certificatemanager/TrustConfig.yaml
#     Template:      https:#github.com/GoogleCloudPlatform/magic-modules/tree/main/mmv1/templates/terraform/resource.html.markdown.tmpl
#
#     DO NOT EDIT this file directly. Any changes made to this file will be
#     overwritten during the next generation cycle.
#
# ----------------------------------------------------------------------------
subcategory: "Certificate Manager"
description: |-
  TrustConfig represents a resource that represents your Public Key Infrastructure (PKI) configuration in Certificate Manager for use in mutual TLS authentication scenarios.
---</rdfs:comment>
  </owl:Class>
  <owl:DatatypeProperty rdf:about="http://example.org/onto/prop/google_certificate_manager_trust_config_create_time">
    <rdfs:label>create_time</rdfs:label>
    <rdfs:comment>The creation timestamp of a TrustConfig.

A timestamp in RFC3339 UTC "Zulu" format, with nanosecond resolution and up to nine fractional digits.
Examples: "2014-10-02T15:01:23Z" and "2014-10-02T15:01:23.045123456Z".</rdfs:comment>
    <rdfs:domain rdf:resource="http://example.org/onto/class/google_certificate_manager_trust_config"/>
    <rdfs:range rdf:resource="http://www.w3.org/2001/XMLSchema#string"/>
  </owl:DatatypeProperty>
  <owl:DatatypeProperty rdf:about="http://example.org/onto/prop/google_certificate_manager_trust_config_description">
    <rdfs:label>description</rdfs:label>
    <rdfs:comment>One or more paragraphs of text description of a trust config.</rdfs:comment>
    <rdfs:domain rdf:resource="http://example.org/onto/class/google_certificate_manager_trust_config"/>
    <rdfs:range rdf:resource="http://www.w3.org/2001/XMLSchema#string"/>
  </owl:DatatypeProperty>
  <owl:DatatypeProperty rdf:about="http://example.org/onto/prop/google_certificate_manager_trust_config_effective_labels">
    <rdfs:label>effective_labels</rdfs:label>
    <rdfs:comment>All of labels (key/value pairs) present on the resource in GCP, including the labels configured through Terraform, other clients and services.</rdfs:comment>
    <rdfs:domain rdf:resource="http://example.org/onto/class/google_certificate_manager_trust_config"/>
    <rdfs:range rdf:resource="http://www.w3.org/2001/XMLSchema#string"/>
  </owl:DatatypeProperty>
  <owl:DatatypeProperty rdf:about="http://example.org/onto/prop/google_certificate_manager_trust_config_id">
    <rdfs:label>id</rdfs:label>
    <rdfs:domain rdf:resource="http://example.org/onto/class/google_certificate_manager_trust_config"/>
    <rdfs:range rdf:resource="http://www.w3.org/2001/XMLSchema#string"/>
  </owl:DatatypeProperty>
  <owl:DatatypeProperty rdf:about="http://example.org/onto/prop/google_certificate_manager_trust_config_labels">
    <rdfs:label>labels</rdfs:label>
    <rdfs:comment>Set of label tags associated with the trust config.

**Note**: This field is non-authoritative, and will only manage the labels present in your configuration.
Please refer to the field 'effective_labels' for all of the labels present on the resource.</rdfs:comment>
    <rdfs:domain rdf:resource="http://example.org/onto/class/google_certificate_manager_trust_config"/>
    <rdfs:range rdf:resource="http://www.w3.org/2001/XMLSchema#string"/>
  </owl:DatatypeProperty>
  <owl:DatatypeProperty rdf:about="http://example.org/onto/prop/google_certificate_manager_trust_config_location">
    <rdfs:label>location</rdfs:label>
    <rdfs:comment>The trust config location.</rdfs:comment>
    <rdfs:domain rdf:resource="http://example.org/onto/class/google_certificate_manager_trust_config"/>
    <rdfs:range rdf:resource="http://www.w3.org/2001/XMLSchema#string"/>
  </owl:DatatypeProperty>
  <owl:DatatypeProperty rdf:about="http://example.org/onto/prop/google_certificate_manager_trust_config_name">
    <rdfs:label>name</rdfs:label>
    <rdfs:comment>A user-defined name of the trust config. Trust config names must be unique globally.</rdfs:comment>
    <rdfs:domain rdf:resource="http://example.org/onto/class/google_certificate_manager_trust_config"/>
    <rdfs:range rdf:resource="http://www.w3.org/2001/XMLSchema#string"/>
  </owl:DatatypeProperty>
  <owl:DatatypeProperty rdf:about="http://example.org/onto/prop/google_certificate_manager_trust_config_project">
    <rdfs:label>project</rdfs:label>
    <rdfs:domain rdf:resource="http://example.org/onto/class/google_certificate_manager_trust_config"/>
    <rdfs:range rdf:resource="http://www.w3.org/2001/XMLSchema#string"/>
  </owl:DatatypeProperty>
  <owl:DatatypeProperty rdf:about="http://example.org/onto/prop/google_certificate_manager_trust_config_terraform_labels">
    <rdfs:label>terraform_labels</rdfs:label>
    <rdfs:comment>The combination of labels configured directly on the resource
 and default labels configured on the provider.</rdfs:comment>
    <rdfs:domain rdf:resource="http://example.org/onto/class/google_certificate_manager_trust_config"/>
    <rdfs:range rdf:resource="http://www.w3.org/2001/XMLSchema#string"/>
  </owl:DatatypeProperty>
  <owl:DatatypeProperty rdf:about="http://example.org/onto/prop/google_certificate_manager_trust_config_update_time">
    <rdfs:label>update_time</rdfs:label>
    <rdfs:comment>The last update timestamp of a TrustConfig.

A timestamp in RFC3339 UTC "Zulu" format, with nanosecond resolution and up to nine fractional digits.
Examples: "2014-10-02T15:01:23Z" and "2014-10-02T15:01:23.045123456Z".</rdfs:comment>
    <rdfs:domain rdf:resource="http://example.org/onto/class/google_certificate_manager_trust_config"/>
    <rdfs:range rdf:resource="http://www.w3.org/2001/XMLSchema#string"/>
  </owl:DatatypeProperty>
  <owl:DatatypeProperty rdf:about="http://example.org/onto/prop/google_certificate_manager_trust_config_pem_certificate">
    <rdfs:label>pem_certificate</rdfs:label>
    <rdfs:comment>PEM certificate that is allowlisted. The certificate can be up to 5k bytes, and must be a parseable X.509 certificate.</rdfs:comment>
    <rdfs:domain rdf:resource="http://example.org/onto/class/google_certificate_manager_trust_config"/>
    <rdfs:range rdf:resource="http://www.w3.org/2001/XMLSchema#string"/>
  </owl:DatatypeProperty>
  <owl:DatatypeProperty rdf:about="http://example.org/onto/prop/google_certificate_manager_trust_config_create">
    <rdfs:label>create</rdfs:label>
    <rdfs:domain rdf:resource="http://example.org/onto/class/google_certificate_manager_trust_config"/>
    <rdfs:range rdf:resource="http://www.w3.org/2001/XMLSchema#string"/>
  </owl:DatatypeProperty>
  <owl:DatatypeProperty rdf:about="http://example.org/onto/prop/google_certificate_manager_trust_config_delete">
    <rdfs:label>delete</rdfs:label>
    <rdfs:domain rdf:resource="http://example.org/onto/class/google_certificate_manager_trust_config"/>
    <rdfs:range rdf:resource="http://www.w3.org/2001/XMLSchema#string"/>
  </owl:DatatypeProperty>
  <owl:DatatypeProperty rdf:about="http://example.org/onto/prop/google_certificate_manager_trust_config_update">
    <rdfs:label>update</rdfs:label>
    <rdfs:domain rdf:resource="http://example.org/onto/class/google_certificate_manager_trust_config"/>
    <rdfs:range rdf:resource="http://www.w3.org/2001/XMLSchema#string"/>
  </owl:DatatypeProperty>
  <owl:DatatypeProperty rdf:about="http://example.org/onto/prop/google_certificate_manager_trust_config_pem_certificate">
    <rdfs:label>pem_certificate</rdfs:label>
    <rdfs:comment>PEM intermediate certificate used for building up paths for validation.
Each certificate provided in PEM format may occupy up to 5kB.</rdfs:comment>
    <rdfs:domain rdf:resource="http://example.org/onto/class/google_certificate_manager_trust_config"/>
    <rdfs:range rdf:resource="http://www.w3.org/2001/XMLSchema#string"/>
  </owl:DatatypeProperty>
  <owl:DatatypeProperty rdf:about="http://example.org/onto/prop/google_certificate_manager_trust_config_pem_certificate">
    <rdfs:label>pem_certificate</rdfs:label>
    <rdfs:comment>PEM root certificate of the PKI used for validation.
Each certificate provided in PEM format may occupy up to 5kB.</rdfs:comment>
    <rdfs:domain rdf:resource="http://example.org/onto/class/google_certificate_manager_trust_config"/>
    <rdfs:range rdf:resource="http://www.w3.org/2001/XMLSchema#string"/>
  </owl:DatatypeProperty>
</rdf:RDF>
