<?xml version="1.0" encoding="UTF-8"?>
<rdf:RDF
  xmlns:rdf="http://www.w3.org/1999/02/22-rdf-syntax-ns#"
  xmlns:rdfs="http://www.w3.org/2000/01/rdf-schema#"
  xmlns:owl="http://www.w3.org/2002/07/owl#"
  xmlns:xsd="http://www.w3.org/2001/XMLSchema#"
  xml:base="http://example.org/onto/">
  <owl:Class rdf:about="http://example.org/onto/class/google_network_connectivity_internal_range">
    <rdfs:label>google_network_connectivity_internal_range</rdfs:label>
    <rdfs:comment>#
#     ***     AUTO GENERATED CODE    ***    Type: MMv1     ***
#
# ----------------------------------------------------------------------------
#
#     This code is generated by Magic Modules using the following:
#
#     Configuration: https:#github.com/GoogleCloudPlatform/magic-modules/tree/main/mmv1/products/networkconnectivityv1/InternalRange.yaml
#     Template:      https:#github.com/GoogleCloudPlatform/magic-modules/tree/main/mmv1/templates/terraform/resource.html.markdown.tmpl
#
#     DO NOT EDIT this file directly. Any changes made to this file will be
#     overwritten during the next generation cycle.
#
# ----------------------------------------------------------------------------
subcategory: "Network Connectivity"
description: |-
  The internal range resource for IPAM operations within a VPC network.
---</rdfs:comment>
  </owl:Class>
  <owl:DatatypeProperty rdf:about="http://example.org/onto/prop/google_network_connectivity_internal_range_description">
    <rdfs:label>description</rdfs:label>
    <rdfs:comment>An optional description of this resource.</rdfs:comment>
    <rdfs:domain rdf:resource="http://example.org/onto/class/google_network_connectivity_internal_range"/>
    <rdfs:range rdf:resource="http://www.w3.org/2001/XMLSchema#string"/>
  </owl:DatatypeProperty>
  <owl:DatatypeProperty rdf:about="http://example.org/onto/prop/google_network_connectivity_internal_range_effective_labels">
    <rdfs:label>effective_labels</rdfs:label>
    <rdfs:comment>All of labels (key/value pairs) present on the resource in GCP, including the labels configured through Terraform, other clients and services.</rdfs:comment>
    <rdfs:domain rdf:resource="http://example.org/onto/class/google_network_connectivity_internal_range"/>
    <rdfs:range rdf:resource="http://www.w3.org/2001/XMLSchema#string"/>
  </owl:DatatypeProperty>
  <owl:DatatypeProperty rdf:about="http://example.org/onto/prop/google_network_connectivity_internal_range_exclude_cidr_ranges">
    <rdfs:label>exclude_cidr_ranges</rdfs:label>
    <rdfs:comment>Optional. List of IP CIDR ranges to be excluded. Resulting reserved Internal Range will not overlap with any CIDR blocks mentioned in this list.
Only IPv4 CIDR ranges are supported.</rdfs:comment>
    <rdfs:domain rdf:resource="http://example.org/onto/class/google_network_connectivity_internal_range"/>
    <rdfs:range rdf:resource="http://www.w3.org/2001/XMLSchema#string"/>
  </owl:DatatypeProperty>
  <owl:DatatypeProperty rdf:about="http://example.org/onto/prop/google_network_connectivity_internal_range_id">
    <rdfs:label>id</rdfs:label>
    <rdfs:domain rdf:resource="http://example.org/onto/class/google_network_connectivity_internal_range"/>
    <rdfs:range rdf:resource="http://www.w3.org/2001/XMLSchema#string"/>
  </owl:DatatypeProperty>
  <owl:DatatypeProperty rdf:about="http://example.org/onto/prop/google_network_connectivity_internal_range_immutable">
    <rdfs:label>immutable</rdfs:label>
    <rdfs:comment>Immutable ranges cannot have their fields modified, except for labels and description.</rdfs:comment>
    <rdfs:domain rdf:resource="http://example.org/onto/class/google_network_connectivity_internal_range"/>
    <rdfs:range rdf:resource="http://www.w3.org/2001/XMLSchema#string"/>
  </owl:DatatypeProperty>
  <owl:DatatypeProperty rdf:about="http://example.org/onto/prop/google_network_connectivity_internal_range_ip_cidr_range">
    <rdfs:label>ip_cidr_range</rdfs:label>
    <rdfs:comment>The IP range that this internal range defines.
NOTE: IPv6 ranges are limited to usage=EXTERNAL_TO_VPC and peering=FOR_SELF
NOTE: For IPv6 Ranges this field is compulsory, i.e. the address range must be specified explicitly.</rdfs:comment>
    <rdfs:domain rdf:resource="http://example.org/onto/class/google_network_connectivity_internal_range"/>
    <rdfs:range rdf:resource="http://www.w3.org/2001/XMLSchema#string"/>
  </owl:DatatypeProperty>
  <owl:DatatypeProperty rdf:about="http://example.org/onto/prop/google_network_connectivity_internal_range_labels">
    <rdfs:label>labels</rdfs:label>
    <rdfs:comment>User-defined labels.


**Note**: This field is non-authoritative, and will only manage the labels present in your configuration.
Please refer to the field 'effective_labels' for all of the labels present on the resource.</rdfs:comment>
    <rdfs:domain rdf:resource="http://example.org/onto/class/google_network_connectivity_internal_range"/>
    <rdfs:range rdf:resource="http://www.w3.org/2001/XMLSchema#string"/>
  </owl:DatatypeProperty>
  <owl:DatatypeProperty rdf:about="http://example.org/onto/prop/google_network_connectivity_internal_range_name">
    <rdfs:label>name</rdfs:label>
    <rdfs:comment>The name of the policy based route.</rdfs:comment>
    <rdfs:domain rdf:resource="http://example.org/onto/class/google_network_connectivity_internal_range"/>
    <rdfs:range rdf:resource="http://www.w3.org/2001/XMLSchema#string"/>
  </owl:DatatypeProperty>
  <owl:DatatypeProperty rdf:about="http://example.org/onto/prop/google_network_connectivity_internal_range_network">
    <rdfs:label>network</rdfs:label>
    <rdfs:comment>Fully-qualified URL of the network that this route applies to, for example: projects/my-project/global/networks/my-network.</rdfs:comment>
    <rdfs:domain rdf:resource="http://example.org/onto/class/google_network_connectivity_internal_range"/>
    <rdfs:range rdf:resource="http://www.w3.org/2001/XMLSchema#string"/>
  </owl:DatatypeProperty>
  <owl:DatatypeProperty rdf:about="http://example.org/onto/prop/google_network_connectivity_internal_range_overlaps">
    <rdfs:label>overlaps</rdfs:label>
    <rdfs:comment>Optional. Types of resources that are allowed to overlap with the current internal range. Possible values: ["OVERLAP_ROUTE_RANGE", "OVERLAP_EXISTING_SUBNET_RANGE"]</rdfs:comment>
    <rdfs:domain rdf:resource="http://example.org/onto/class/google_network_connectivity_internal_range"/>
    <rdfs:range rdf:resource="http://www.w3.org/2001/XMLSchema#string"/>
  </owl:DatatypeProperty>
  <owl:DatatypeProperty rdf:about="http://example.org/onto/prop/google_network_connectivity_internal_range_peering">
    <rdfs:label>peering</rdfs:label>
    <rdfs:comment>The type of peering set for this internal range. Possible values: ["FOR_SELF", "FOR_PEER", "NOT_SHARED"]</rdfs:comment>
    <rdfs:domain rdf:resource="http://example.org/onto/class/google_network_connectivity_internal_range"/>
    <rdfs:range rdf:resource="http://www.w3.org/2001/XMLSchema#string"/>
  </owl:DatatypeProperty>
  <owl:DatatypeProperty rdf:about="http://example.org/onto/prop/google_network_connectivity_internal_range_prefix_length">
    <rdfs:label>prefix_length</rdfs:label>
    <rdfs:comment>An alternate to ipCidrRange. Can be set when trying to create a reservation that automatically finds a free range of the given size.
If both ipCidrRange and prefixLength are set, there is an error if the range sizes do not match. Can also be used during updates to change the range size.
NOTE: For IPv6 this field only works if ip_cidr_range is set as well, and both fields must match. In other words, with IPv6 this field only works as
a redundant parameter.</rdfs:comment>
    <rdfs:domain rdf:resource="http://example.org/onto/class/google_network_connectivity_internal_range"/>
    <rdfs:range rdf:resource="http://www.w3.org/2001/XMLSchema#string"/>
  </owl:DatatypeProperty>
  <owl:DatatypeProperty rdf:about="http://example.org/onto/prop/google_network_connectivity_internal_range_project">
    <rdfs:label>project</rdfs:label>
    <rdfs:domain rdf:resource="http://example.org/onto/class/google_network_connectivity_internal_range"/>
    <rdfs:range rdf:resource="http://www.w3.org/2001/XMLSchema#string"/>
  </owl:DatatypeProperty>
  <owl:DatatypeProperty rdf:about="http://example.org/onto/prop/google_network_connectivity_internal_range_target_cidr_range">
    <rdfs:label>target_cidr_range</rdfs:label>
    <rdfs:comment>Optional. Can be set to narrow down or pick a different address space while searching for a free range.
If not set, defaults to the "10.0.0.0/8" address space. This can be used to search in other rfc-1918 address spaces like "172.16.0.0/12" and "192.168.0.0/16" or non-rfc-1918 address spaces used in the VPC.</rdfs:comment>
    <rdfs:domain rdf:resource="http://example.org/onto/class/google_network_connectivity_internal_range"/>
    <rdfs:range rdf:resource="http://www.w3.org/2001/XMLSchema#string"/>
  </owl:DatatypeProperty>
  <owl:DatatypeProperty rdf:about="http://example.org/onto/prop/google_network_connectivity_internal_range_terraform_labels">
    <rdfs:label>terraform_labels</rdfs:label>
    <rdfs:comment>The combination of labels configured directly on the resource
 and default labels configured on the provider.</rdfs:comment>
    <rdfs:domain rdf:resource="http://example.org/onto/class/google_network_connectivity_internal_range"/>
    <rdfs:range rdf:resource="http://www.w3.org/2001/XMLSchema#string"/>
  </owl:DatatypeProperty>
  <owl:DatatypeProperty rdf:about="http://example.org/onto/prop/google_network_connectivity_internal_range_usage">
    <rdfs:label>usage</rdfs:label>
    <rdfs:comment>The type of usage set for this InternalRange. Possible values: ["FOR_VPC", "EXTERNAL_TO_VPC", "FOR_MIGRATION"]</rdfs:comment>
    <rdfs:domain rdf:resource="http://example.org/onto/class/google_network_connectivity_internal_range"/>
    <rdfs:range rdf:resource="http://www.w3.org/2001/XMLSchema#string"/>
  </owl:DatatypeProperty>
  <owl:DatatypeProperty rdf:about="http://example.org/onto/prop/google_network_connectivity_internal_range_users">
    <rdfs:label>users</rdfs:label>
    <rdfs:comment>Output only. The list of resources that refer to this internal range.
Resources that use the internal range for their range allocation are referred to as users of the range.
Other resources mark themselves as users while doing so by creating a reference to this internal range. Having a user, based on this reference, prevents deletion of the internal range referred to. Can be empty.</rdfs:comment>
    <rdfs:domain rdf:resource="http://example.org/onto/class/google_network_connectivity_internal_range"/>
    <rdfs:range rdf:resource="http://www.w3.org/2001/XMLSchema#string"/>
  </owl:DatatypeProperty>
  <owl:DatatypeProperty rdf:about="http://example.org/onto/prop/google_network_connectivity_internal_range_allocation_strategy">
    <rdfs:label>allocation_strategy</rdfs:label>
    <rdfs:comment>Optional. Sets the strategy used to automatically find a free range of a size given by prefixLength. Can be set only when trying to create a reservation that automatically finds the free range to reserve. Possible values: ["RANDOM", "FIRST_AVAILABLE", "RANDOM_FIRST_N_AVAILABLE", "FIRST_SMALLEST_FITTING"]</rdfs:comment>
    <rdfs:domain rdf:resource="http://example.org/onto/class/google_network_connectivity_internal_range"/>
    <rdfs:range rdf:resource="http://www.w3.org/2001/XMLSchema#string"/>
  </owl:DatatypeProperty>
  <owl:DatatypeProperty rdf:about="http://example.org/onto/prop/google_network_connectivity_internal_range_first_available_ranges_lookup_size">
    <rdfs:label>first_available_ranges_lookup_size</rdfs:label>
    <rdfs:comment>Must be set when allocation_strategy is RANDOM_FIRST_N_AVAILABLE, otherwise must remain unset. Defines the size of the set of free ranges from which RANDOM_FIRST_N_AVAILABLE strategy randomy selects one,
in other words it sets the N in the RANDOM_FIRST_N_AVAILABLE.</rdfs:comment>
    <rdfs:domain rdf:resource="http://example.org/onto/class/google_network_connectivity_internal_range"/>
    <rdfs:range rdf:resource="http://www.w3.org/2001/XMLSchema#string"/>
  </owl:DatatypeProperty>
  <owl:DatatypeProperty rdf:about="http://example.org/onto/prop/google_network_connectivity_internal_range_source">
    <rdfs:label>source</rdfs:label>
    <rdfs:comment>Resource path as an URI of the source resource, for example a subnet.
The project for the source resource should match the project for the
InternalRange.
An example /projects/{project}/regions/{region}/subnetworks/{subnet}</rdfs:comment>
    <rdfs:domain rdf:resource="http://example.org/onto/class/google_network_connectivity_internal_range"/>
    <rdfs:range rdf:resource="http://www.w3.org/2001/XMLSchema#string"/>
  </owl:DatatypeProperty>
  <owl:DatatypeProperty rdf:about="http://example.org/onto/prop/google_network_connectivity_internal_range_target">
    <rdfs:label>target</rdfs:label>
    <rdfs:comment>Resource path of the target resource. The target project can be
different, as in the cases when migrating to peer networks. The resource
may not exist yet.
For example /projects/{project}/regions/{region}/subnetworks/{subnet}</rdfs:comment>
    <rdfs:domain rdf:resource="http://example.org/onto/class/google_network_connectivity_internal_range"/>
    <rdfs:range rdf:resource="http://www.w3.org/2001/XMLSchema#string"/>
  </owl:DatatypeProperty>
  <owl:DatatypeProperty rdf:about="http://example.org/onto/prop/google_network_connectivity_internal_range_create">
    <rdfs:label>create</rdfs:label>
    <rdfs:domain rdf:resource="http://example.org/onto/class/google_network_connectivity_internal_range"/>
    <rdfs:range rdf:resource="http://www.w3.org/2001/XMLSchema#string"/>
  </owl:DatatypeProperty>
  <owl:DatatypeProperty rdf:about="http://example.org/onto/prop/google_network_connectivity_internal_range_delete">
    <rdfs:label>delete</rdfs:label>
    <rdfs:domain rdf:resource="http://example.org/onto/class/google_network_connectivity_internal_range"/>
    <rdfs:range rdf:resource="http://www.w3.org/2001/XMLSchema#string"/>
  </owl:DatatypeProperty>
  <owl:DatatypeProperty rdf:about="http://example.org/onto/prop/google_network_connectivity_internal_range_update">
    <rdfs:label>update</rdfs:label>
    <rdfs:domain rdf:resource="http://example.org/onto/class/google_network_connectivity_internal_range"/>
    <rdfs:range rdf:resource="http://www.w3.org/2001/XMLSchema#string"/>
  </owl:DatatypeProperty>
</rdf:RDF>
