<?xml version="1.0" encoding="UTF-8"?>
<rdf:RDF
  xmlns:rdf="http://www.w3.org/1999/02/22-rdf-syntax-ns#"
  xmlns:rdfs="http://www.w3.org/2000/01/rdf-schema#"
  xmlns:owl="http://www.w3.org/2002/07/owl#"
  xmlns:xsd="http://www.w3.org/2001/XMLSchema#"
  xml:base="http://example.org/onto/">
  <owl:Class rdf:about="http://example.org/onto/class/google_bigquery_dataset">
    <rdfs:label>google_bigquery_dataset</rdfs:label>
    <rdfs:comment>#
#     ***     AUTO GENERATED CODE    ***    Type: MMv1     ***
#
# ----------------------------------------------------------------------------
#
#     This code is generated by Magic Modules using the following:
#
#     Configuration: https:#github.com/GoogleCloudPlatform/magic-modules/tree/main/mmv1/products/bigquery/Dataset.yaml
#     Template:      https:#github.com/GoogleCloudPlatform/magic-modules/tree/main/mmv1/templates/terraform/resource.html.markdown.tmpl
#
#     DO NOT EDIT this file directly. Any changes made to this file will be
#     overwritten during the next generation cycle.
#
# ----------------------------------------------------------------------------
subcategory: "BigQuery"
description: |-
  Datasets allow you to organize and control access to your tables.
---</rdfs:comment>
  </owl:Class>
  <owl:DatatypeProperty rdf:about="http://example.org/onto/prop/google_bigquery_dataset_creation_time">
    <rdfs:label>creation_time</rdfs:label>
    <rdfs:comment>The time when this dataset was created, in milliseconds since the
epoch.</rdfs:comment>
    <rdfs:domain rdf:resource="http://example.org/onto/class/google_bigquery_dataset"/>
    <rdfs:range rdf:resource="http://www.w3.org/2001/XMLSchema#string"/>
  </owl:DatatypeProperty>
  <owl:DatatypeProperty rdf:about="http://example.org/onto/prop/google_bigquery_dataset_dataset_id">
    <rdfs:label>dataset_id</rdfs:label>
    <rdfs:comment>A unique ID for this dataset, without the project name. The ID
must contain only letters (a-z, A-Z), numbers (0-9), or
underscores (_). The maximum length is 1,024 characters.</rdfs:comment>
    <rdfs:domain rdf:resource="http://example.org/onto/class/google_bigquery_dataset"/>
    <rdfs:range rdf:resource="http://www.w3.org/2001/XMLSchema#string"/>
  </owl:DatatypeProperty>
  <owl:DatatypeProperty rdf:about="http://example.org/onto/prop/google_bigquery_dataset_default_collation">
    <rdfs:label>default_collation</rdfs:label>
    <rdfs:comment>Defines the default collation specification of future tables created
in the dataset. If a table is created in this dataset without table-level
default collation, then the table inherits the dataset default collation,
which is applied to the string fields that do not have explicit collation
specified. A change to this field affects only tables created afterwards,
and does not alter the existing tables.

The following values are supported:
- 'und:ci': undetermined locale, case insensitive.
- '': empty string. Default to case-sensitive behavior.</rdfs:comment>
    <rdfs:domain rdf:resource="http://example.org/onto/class/google_bigquery_dataset"/>
    <rdfs:range rdf:resource="http://www.w3.org/2001/XMLSchema#string"/>
  </owl:DatatypeProperty>
  <owl:DatatypeProperty rdf:about="http://example.org/onto/prop/google_bigquery_dataset_default_partition_expiration_ms">
    <rdfs:label>default_partition_expiration_ms</rdfs:label>
    <rdfs:comment>The default partition expiration for all partitioned tables in
the dataset, in milliseconds.
Once this property is set, all newly-created partitioned tables in
the dataset will have an 'expirationMs' property in the 'timePartitioning'
settings set to this value, and changing the value will only
affect new tables, not existing ones. The storage in a partition will
have an expiration time of its partition time plus this value.
Setting this property overrides the use of 'defaultTableExpirationMs'
for partitioned tables: only one of 'defaultTableExpirationMs' and
'defaultPartitionExpirationMs' will be used for any new partitioned
table. If you provide an explicit 'timePartitioning.expirationMs' when
creating or updating a partitioned table, that value takes precedence
over the default partition expiration time indicated by this property.</rdfs:comment>
    <rdfs:domain rdf:resource="http://example.org/onto/class/google_bigquery_dataset"/>
    <rdfs:range rdf:resource="http://www.w3.org/2001/XMLSchema#string"/>
  </owl:DatatypeProperty>
  <owl:DatatypeProperty rdf:about="http://example.org/onto/prop/google_bigquery_dataset_default_table_expiration_ms">
    <rdfs:label>default_table_expiration_ms</rdfs:label>
    <rdfs:comment>The default lifetime of all tables in the dataset, in milliseconds.
The minimum value is 3600000 milliseconds (one hour).
Once this property is set, all newly-created tables in the dataset
will have an 'expirationTime' property set to the creation time plus
the value in this property, and changing the value will only affect
new tables, not existing ones. When the 'expirationTime' for a given
table is reached, that table will be deleted automatically.
If a table's 'expirationTime' is modified or removed before the
table expires, or if you provide an explicit 'expirationTime' when
creating a table, that value takes precedence over the default
expiration time indicated by this property.</rdfs:comment>
    <rdfs:domain rdf:resource="http://example.org/onto/class/google_bigquery_dataset"/>
    <rdfs:range rdf:resource="http://www.w3.org/2001/XMLSchema#string"/>
  </owl:DatatypeProperty>
  <owl:DatatypeProperty rdf:about="http://example.org/onto/prop/google_bigquery_dataset_delete_contents_on_destroy">
    <rdfs:label>delete_contents_on_destroy</rdfs:label>
    <rdfs:comment>If set to 'true', delete all the tables in the
dataset when destroying the resource; otherwise,
destroying the resource will fail if tables are present.</rdfs:comment>
    <rdfs:domain rdf:resource="http://example.org/onto/class/google_bigquery_dataset"/>
    <rdfs:range rdf:resource="http://www.w3.org/2001/XMLSchema#string"/>
  </owl:DatatypeProperty>
  <owl:DatatypeProperty rdf:about="http://example.org/onto/prop/google_bigquery_dataset_description">
    <rdfs:label>description</rdfs:label>
    <rdfs:comment>A user-friendly description of the dataset</rdfs:comment>
    <rdfs:domain rdf:resource="http://example.org/onto/class/google_bigquery_dataset"/>
    <rdfs:range rdf:resource="http://www.w3.org/2001/XMLSchema#string"/>
  </owl:DatatypeProperty>
  <owl:DatatypeProperty rdf:about="http://example.org/onto/prop/google_bigquery_dataset_effective_labels">
    <rdfs:label>effective_labels</rdfs:label>
    <rdfs:comment>All of labels (key/value pairs) present on the resource in GCP, including the labels configured through Terraform, other clients and services.</rdfs:comment>
    <rdfs:domain rdf:resource="http://example.org/onto/class/google_bigquery_dataset"/>
    <rdfs:range rdf:resource="http://www.w3.org/2001/XMLSchema#string"/>
  </owl:DatatypeProperty>
  <owl:DatatypeProperty rdf:about="http://example.org/onto/prop/google_bigquery_dataset_etag">
    <rdfs:label>etag</rdfs:label>
    <rdfs:comment>A hash of the resource.</rdfs:comment>
    <rdfs:domain rdf:resource="http://example.org/onto/class/google_bigquery_dataset"/>
    <rdfs:range rdf:resource="http://www.w3.org/2001/XMLSchema#string"/>
  </owl:DatatypeProperty>
  <owl:DatatypeProperty rdf:about="http://example.org/onto/prop/google_bigquery_dataset_friendly_name">
    <rdfs:label>friendly_name</rdfs:label>
    <rdfs:comment>A descriptive name for the dataset</rdfs:comment>
    <rdfs:domain rdf:resource="http://example.org/onto/class/google_bigquery_dataset"/>
    <rdfs:range rdf:resource="http://www.w3.org/2001/XMLSchema#string"/>
  </owl:DatatypeProperty>
  <owl:DatatypeProperty rdf:about="http://example.org/onto/prop/google_bigquery_dataset_id">
    <rdfs:label>id</rdfs:label>
    <rdfs:domain rdf:resource="http://example.org/onto/class/google_bigquery_dataset"/>
    <rdfs:range rdf:resource="http://www.w3.org/2001/XMLSchema#string"/>
  </owl:DatatypeProperty>
  <owl:DatatypeProperty rdf:about="http://example.org/onto/prop/google_bigquery_dataset_is_case_insensitive">
    <rdfs:label>is_case_insensitive</rdfs:label>
    <rdfs:comment>TRUE if the dataset and its table names are case-insensitive, otherwise FALSE.
By default, this is FALSE, which means the dataset and its table names are
case-sensitive. This field does not affect routine references.</rdfs:comment>
    <rdfs:domain rdf:resource="http://example.org/onto/class/google_bigquery_dataset"/>
    <rdfs:range rdf:resource="http://www.w3.org/2001/XMLSchema#string"/>
  </owl:DatatypeProperty>
  <owl:DatatypeProperty rdf:about="http://example.org/onto/prop/google_bigquery_dataset_labels">
    <rdfs:label>labels</rdfs:label>
    <rdfs:comment>The labels associated with this dataset. You can use these to
organize and group your datasets.


**Note**: This field is non-authoritative, and will only manage the labels present in your configuration.
Please refer to the field 'effective_labels' for all of the labels present on the resource.</rdfs:comment>
    <rdfs:domain rdf:resource="http://example.org/onto/class/google_bigquery_dataset"/>
    <rdfs:range rdf:resource="http://www.w3.org/2001/XMLSchema#string"/>
  </owl:DatatypeProperty>
  <owl:DatatypeProperty rdf:about="http://example.org/onto/prop/google_bigquery_dataset_last_modified_time">
    <rdfs:label>last_modified_time</rdfs:label>
    <rdfs:comment>The date when this dataset or any of its tables was last modified, in
milliseconds since the epoch.</rdfs:comment>
    <rdfs:domain rdf:resource="http://example.org/onto/class/google_bigquery_dataset"/>
    <rdfs:range rdf:resource="http://www.w3.org/2001/XMLSchema#string"/>
  </owl:DatatypeProperty>
  <owl:DatatypeProperty rdf:about="http://example.org/onto/prop/google_bigquery_dataset_location">
    <rdfs:label>location</rdfs:label>
    <rdfs:comment>The geographic location where the dataset should reside.
See [official docs](https://cloud.google.com/bigquery/docs/dataset-locations).
There are two types of locations, regional or multi-regional. A regional
location is a specific geographic place, such as Tokyo, and a multi-regional
location is a large geographic area, such as the United States, that
contains at least two geographic places.
The default value is multi-regional location 'US'.
Changing this forces a new resource to be created.</rdfs:comment>
    <rdfs:domain rdf:resource="http://example.org/onto/class/google_bigquery_dataset"/>
    <rdfs:range rdf:resource="http://www.w3.org/2001/XMLSchema#string"/>
  </owl:DatatypeProperty>
  <owl:DatatypeProperty rdf:about="http://example.org/onto/prop/google_bigquery_dataset_max_time_travel_hours">
    <rdfs:label>max_time_travel_hours</rdfs:label>
    <rdfs:comment>Defines the time travel window in hours. The value can be from 48 to 168 hours (2 to 7 days).</rdfs:comment>
    <rdfs:domain rdf:resource="http://example.org/onto/class/google_bigquery_dataset"/>
    <rdfs:range rdf:resource="http://www.w3.org/2001/XMLSchema#string"/>
  </owl:DatatypeProperty>
  <owl:DatatypeProperty rdf:about="http://example.org/onto/prop/google_bigquery_dataset_project">
    <rdfs:label>project</rdfs:label>
    <rdfs:domain rdf:resource="http://example.org/onto/class/google_bigquery_dataset"/>
    <rdfs:range rdf:resource="http://www.w3.org/2001/XMLSchema#string"/>
  </owl:DatatypeProperty>
  <owl:DatatypeProperty rdf:about="http://example.org/onto/prop/google_bigquery_dataset_resource_tags">
    <rdfs:label>resource_tags</rdfs:label>
    <rdfs:comment>The tags attached to this table. Tag keys are globally unique. Tag key is expected to be
in the namespaced format, for example "123456789012/environment" where 123456789012 is the
ID of the parent organization or project resource for this tag key. Tag value is expected
to be the short name, for example "Production". See [Tag definitions](https://cloud.google.com/iam/docs/tags-access-control#definitions)
for more details.</rdfs:comment>
    <rdfs:domain rdf:resource="http://example.org/onto/class/google_bigquery_dataset"/>
    <rdfs:range rdf:resource="http://www.w3.org/2001/XMLSchema#string"/>
  </owl:DatatypeProperty>
  <owl:DatatypeProperty rdf:about="http://example.org/onto/prop/google_bigquery_dataset_self_link">
    <rdfs:label>self_link</rdfs:label>
    <rdfs:domain rdf:resource="http://example.org/onto/class/google_bigquery_dataset"/>
    <rdfs:range rdf:resource="http://www.w3.org/2001/XMLSchema#string"/>
  </owl:DatatypeProperty>
  <owl:DatatypeProperty rdf:about="http://example.org/onto/prop/google_bigquery_dataset_storage_billing_model">
    <rdfs:label>storage_billing_model</rdfs:label>
    <rdfs:comment>Specifies the storage billing model for the dataset.
Set this flag value to LOGICAL to use logical bytes for storage billing,
or to PHYSICAL to use physical bytes instead.

LOGICAL is the default if this flag isn't specified.</rdfs:comment>
    <rdfs:domain rdf:resource="http://example.org/onto/class/google_bigquery_dataset"/>
    <rdfs:range rdf:resource="http://www.w3.org/2001/XMLSchema#string"/>
  </owl:DatatypeProperty>
  <owl:DatatypeProperty rdf:about="http://example.org/onto/prop/google_bigquery_dataset_terraform_labels">
    <rdfs:label>terraform_labels</rdfs:label>
    <rdfs:comment>The combination of labels configured directly on the resource
 and default labels configured on the provider.</rdfs:comment>
    <rdfs:domain rdf:resource="http://example.org/onto/class/google_bigquery_dataset"/>
    <rdfs:range rdf:resource="http://www.w3.org/2001/XMLSchema#string"/>
  </owl:DatatypeProperty>
  <owl:DatatypeProperty rdf:about="http://example.org/onto/prop/google_bigquery_dataset_domain">
    <rdfs:label>domain</rdfs:label>
    <rdfs:comment>A domain to grant access to. Any users signed in with the
domain specified will be granted the specified access</rdfs:comment>
    <rdfs:domain rdf:resource="http://example.org/onto/class/google_bigquery_dataset"/>
    <rdfs:range rdf:resource="http://www.w3.org/2001/XMLSchema#string"/>
  </owl:DatatypeProperty>
  <owl:DatatypeProperty rdf:about="http://example.org/onto/prop/google_bigquery_dataset_group_by_email">
    <rdfs:label>group_by_email</rdfs:label>
    <rdfs:comment>An email address of a Google Group to grant access to.</rdfs:comment>
    <rdfs:domain rdf:resource="http://example.org/onto/class/google_bigquery_dataset"/>
    <rdfs:range rdf:resource="http://www.w3.org/2001/XMLSchema#string"/>
  </owl:DatatypeProperty>
  <owl:DatatypeProperty rdf:about="http://example.org/onto/prop/google_bigquery_dataset_iam_member">
    <rdfs:label>iam_member</rdfs:label>
    <rdfs:comment>Some other type of member that appears in the IAM Policy but isn't a user,
group, domain, or special group. For example: 'allUsers'</rdfs:comment>
    <rdfs:domain rdf:resource="http://example.org/onto/class/google_bigquery_dataset"/>
    <rdfs:range rdf:resource="http://www.w3.org/2001/XMLSchema#string"/>
  </owl:DatatypeProperty>
  <owl:DatatypeProperty rdf:about="http://example.org/onto/prop/google_bigquery_dataset_role">
    <rdfs:label>role</rdfs:label>
    <rdfs:comment>Describes the rights granted to the user specified by the other
member of the access object. Basic, predefined, and custom roles
are supported. Predefined roles that have equivalent basic roles
are swapped by the API to their basic counterparts. See
[official docs](https://cloud.google.com/bigquery/docs/access-control).</rdfs:comment>
    <rdfs:domain rdf:resource="http://example.org/onto/class/google_bigquery_dataset"/>
    <rdfs:range rdf:resource="http://www.w3.org/2001/XMLSchema#string"/>
  </owl:DatatypeProperty>
  <owl:DatatypeProperty rdf:about="http://example.org/onto/prop/google_bigquery_dataset_special_group">
    <rdfs:label>special_group</rdfs:label>
    <rdfs:comment>A special group to grant access to. Possible values include:
* 'projectOwners': Owners of the enclosing project.
* 'projectReaders': Readers of the enclosing project.
* 'projectWriters': Writers of the enclosing project.
* 'allAuthenticatedUsers': All authenticated BigQuery users.</rdfs:comment>
    <rdfs:domain rdf:resource="http://example.org/onto/class/google_bigquery_dataset"/>
    <rdfs:range rdf:resource="http://www.w3.org/2001/XMLSchema#string"/>
  </owl:DatatypeProperty>
  <owl:DatatypeProperty rdf:about="http://example.org/onto/prop/google_bigquery_dataset_user_by_email">
    <rdfs:label>user_by_email</rdfs:label>
    <rdfs:comment>An email address of a user to grant access to. For example:
fred@example.com</rdfs:comment>
    <rdfs:domain rdf:resource="http://example.org/onto/class/google_bigquery_dataset"/>
    <rdfs:range rdf:resource="http://www.w3.org/2001/XMLSchema#string"/>
  </owl:DatatypeProperty>
  <owl:DatatypeProperty rdf:about="http://example.org/onto/prop/google_bigquery_dataset_description">
    <rdfs:label>description</rdfs:label>
    <rdfs:comment>Description of the expression. This is a longer text which describes the expression,
e.g. when hovered over it in a UI.</rdfs:comment>
    <rdfs:domain rdf:resource="http://example.org/onto/class/google_bigquery_dataset"/>
    <rdfs:range rdf:resource="http://www.w3.org/2001/XMLSchema#string"/>
  </owl:DatatypeProperty>
  <owl:DatatypeProperty rdf:about="http://example.org/onto/prop/google_bigquery_dataset_expression">
    <rdfs:label>expression</rdfs:label>
    <rdfs:comment>Textual representation of an expression in Common Expression Language syntax.</rdfs:comment>
    <rdfs:domain rdf:resource="http://example.org/onto/class/google_bigquery_dataset"/>
    <rdfs:range rdf:resource="http://www.w3.org/2001/XMLSchema#string"/>
  </owl:DatatypeProperty>
  <owl:DatatypeProperty rdf:about="http://example.org/onto/prop/google_bigquery_dataset_location">
    <rdfs:label>location</rdfs:label>
    <rdfs:comment>String indicating the location of the expression for error reporting, e.g. a file
name and a position in the file.</rdfs:comment>
    <rdfs:domain rdf:resource="http://example.org/onto/class/google_bigquery_dataset"/>
    <rdfs:range rdf:resource="http://www.w3.org/2001/XMLSchema#string"/>
  </owl:DatatypeProperty>
  <owl:DatatypeProperty rdf:about="http://example.org/onto/prop/google_bigquery_dataset_title">
    <rdfs:label>title</rdfs:label>
    <rdfs:comment>Title for the expression, i.e. a short string describing its purpose.
This can be used e.g. in UIs which allow to enter the expression.</rdfs:comment>
    <rdfs:domain rdf:resource="http://example.org/onto/class/google_bigquery_dataset"/>
    <rdfs:range rdf:resource="http://www.w3.org/2001/XMLSchema#string"/>
  </owl:DatatypeProperty>
  <owl:DatatypeProperty rdf:about="http://example.org/onto/prop/google_bigquery_dataset_target_types">
    <rdfs:label>target_types</rdfs:label>
    <rdfs:comment>Which resources in the dataset this entry applies to. Currently, only views are supported,
but additional target types may be added in the future. Possible values: VIEWS</rdfs:comment>
    <rdfs:domain rdf:resource="http://example.org/onto/class/google_bigquery_dataset"/>
    <rdfs:range rdf:resource="http://www.w3.org/2001/XMLSchema#string"/>
  </owl:DatatypeProperty>
  <owl:DatatypeProperty rdf:about="http://example.org/onto/prop/google_bigquery_dataset_dataset_id">
    <rdfs:label>dataset_id</rdfs:label>
    <rdfs:comment>The ID of the dataset containing this table.</rdfs:comment>
    <rdfs:domain rdf:resource="http://example.org/onto/class/google_bigquery_dataset"/>
    <rdfs:range rdf:resource="http://www.w3.org/2001/XMLSchema#string"/>
  </owl:DatatypeProperty>
  <owl:DatatypeProperty rdf:about="http://example.org/onto/prop/google_bigquery_dataset_project_id">
    <rdfs:label>project_id</rdfs:label>
    <rdfs:comment>The ID of the project containing this table.</rdfs:comment>
    <rdfs:domain rdf:resource="http://example.org/onto/class/google_bigquery_dataset"/>
    <rdfs:range rdf:resource="http://www.w3.org/2001/XMLSchema#string"/>
  </owl:DatatypeProperty>
  <owl:DatatypeProperty rdf:about="http://example.org/onto/prop/google_bigquery_dataset_dataset_id">
    <rdfs:label>dataset_id</rdfs:label>
    <rdfs:comment>The ID of the dataset containing this table.</rdfs:comment>
    <rdfs:domain rdf:resource="http://example.org/onto/class/google_bigquery_dataset"/>
    <rdfs:range rdf:resource="http://www.w3.org/2001/XMLSchema#string"/>
  </owl:DatatypeProperty>
  <owl:DatatypeProperty rdf:about="http://example.org/onto/prop/google_bigquery_dataset_project_id">
    <rdfs:label>project_id</rdfs:label>
    <rdfs:comment>The ID of the project containing this table.</rdfs:comment>
    <rdfs:domain rdf:resource="http://example.org/onto/class/google_bigquery_dataset"/>
    <rdfs:range rdf:resource="http://www.w3.org/2001/XMLSchema#string"/>
  </owl:DatatypeProperty>
  <owl:DatatypeProperty rdf:about="http://example.org/onto/prop/google_bigquery_dataset_routine_id">
    <rdfs:label>routine_id</rdfs:label>
    <rdfs:comment>The ID of the routine. The ID must contain only letters (a-z,
A-Z), numbers (0-9), or underscores (_). The maximum length
is 256 characters.</rdfs:comment>
    <rdfs:domain rdf:resource="http://example.org/onto/class/google_bigquery_dataset"/>
    <rdfs:range rdf:resource="http://www.w3.org/2001/XMLSchema#string"/>
  </owl:DatatypeProperty>
  <owl:DatatypeProperty rdf:about="http://example.org/onto/prop/google_bigquery_dataset_dataset_id">
    <rdfs:label>dataset_id</rdfs:label>
    <rdfs:comment>The ID of the dataset containing this table.</rdfs:comment>
    <rdfs:domain rdf:resource="http://example.org/onto/class/google_bigquery_dataset"/>
    <rdfs:range rdf:resource="http://www.w3.org/2001/XMLSchema#string"/>
  </owl:DatatypeProperty>
  <owl:DatatypeProperty rdf:about="http://example.org/onto/prop/google_bigquery_dataset_project_id">
    <rdfs:label>project_id</rdfs:label>
    <rdfs:comment>The ID of the project containing this table.</rdfs:comment>
    <rdfs:domain rdf:resource="http://example.org/onto/class/google_bigquery_dataset"/>
    <rdfs:range rdf:resource="http://www.w3.org/2001/XMLSchema#string"/>
  </owl:DatatypeProperty>
  <owl:DatatypeProperty rdf:about="http://example.org/onto/prop/google_bigquery_dataset_table_id">
    <rdfs:label>table_id</rdfs:label>
    <rdfs:comment>The ID of the table. The ID must contain only letters (a-z,
A-Z), numbers (0-9), or underscores (_). The maximum length
is 1,024 characters.</rdfs:comment>
    <rdfs:domain rdf:resource="http://example.org/onto/class/google_bigquery_dataset"/>
    <rdfs:range rdf:resource="http://www.w3.org/2001/XMLSchema#string"/>
  </owl:DatatypeProperty>
  <owl:DatatypeProperty rdf:about="http://example.org/onto/prop/google_bigquery_dataset_kms_key_name">
    <rdfs:label>kms_key_name</rdfs:label>
    <rdfs:comment>Describes the Cloud KMS encryption key that will be used to protect destination
BigQuery table. The BigQuery Service Account associated with your project requires
access to this encryption key.</rdfs:comment>
    <rdfs:domain rdf:resource="http://example.org/onto/class/google_bigquery_dataset"/>
    <rdfs:range rdf:resource="http://www.w3.org/2001/XMLSchema#string"/>
  </owl:DatatypeProperty>
  <owl:DatatypeProperty rdf:about="http://example.org/onto/prop/google_bigquery_dataset_default_storage_location_uri">
    <rdfs:label>default_storage_location_uri</rdfs:label>
    <rdfs:comment>The storage location URI for all tables in the dataset. Equivalent to hive metastore's
database locationUri. Maximum length of 1024 characters.</rdfs:comment>
    <rdfs:domain rdf:resource="http://example.org/onto/class/google_bigquery_dataset"/>
    <rdfs:range rdf:resource="http://www.w3.org/2001/XMLSchema#string"/>
  </owl:DatatypeProperty>
  <owl:DatatypeProperty rdf:about="http://example.org/onto/prop/google_bigquery_dataset_parameters">
    <rdfs:label>parameters</rdfs:label>
    <rdfs:comment>A map of key value pairs defining the parameters and properties of the open source schema.
Maximum size of 2Mib.</rdfs:comment>
    <rdfs:domain rdf:resource="http://example.org/onto/class/google_bigquery_dataset"/>
    <rdfs:range rdf:resource="http://www.w3.org/2001/XMLSchema#string"/>
  </owl:DatatypeProperty>
  <owl:DatatypeProperty rdf:about="http://example.org/onto/prop/google_bigquery_dataset_connection">
    <rdfs:label>connection</rdfs:label>
    <rdfs:comment>The connection id that is used to access the externalSource.
Format: projects/{projectId}/locations/{locationId}/connections/{connectionId}</rdfs:comment>
    <rdfs:domain rdf:resource="http://example.org/onto/class/google_bigquery_dataset"/>
    <rdfs:range rdf:resource="http://www.w3.org/2001/XMLSchema#string"/>
  </owl:DatatypeProperty>
  <owl:DatatypeProperty rdf:about="http://example.org/onto/prop/google_bigquery_dataset_external_source">
    <rdfs:label>external_source</rdfs:label>
    <rdfs:comment>External source that backs this dataset.</rdfs:comment>
    <rdfs:domain rdf:resource="http://example.org/onto/class/google_bigquery_dataset"/>
    <rdfs:range rdf:resource="http://www.w3.org/2001/XMLSchema#string"/>
  </owl:DatatypeProperty>
  <owl:DatatypeProperty rdf:about="http://example.org/onto/prop/google_bigquery_dataset_create">
    <rdfs:label>create</rdfs:label>
    <rdfs:domain rdf:resource="http://example.org/onto/class/google_bigquery_dataset"/>
    <rdfs:range rdf:resource="http://www.w3.org/2001/XMLSchema#string"/>
  </owl:DatatypeProperty>
  <owl:DatatypeProperty rdf:about="http://example.org/onto/prop/google_bigquery_dataset_delete">
    <rdfs:label>delete</rdfs:label>
    <rdfs:domain rdf:resource="http://example.org/onto/class/google_bigquery_dataset"/>
    <rdfs:range rdf:resource="http://www.w3.org/2001/XMLSchema#string"/>
  </owl:DatatypeProperty>
  <owl:DatatypeProperty rdf:about="http://example.org/onto/prop/google_bigquery_dataset_update">
    <rdfs:label>update</rdfs:label>
    <rdfs:domain rdf:resource="http://example.org/onto/class/google_bigquery_dataset"/>
    <rdfs:range rdf:resource="http://www.w3.org/2001/XMLSchema#string"/>
  </owl:DatatypeProperty>
</rdf:RDF>
