<?xml version="1.0" encoding="UTF-8"?>
<rdf:RDF
  xmlns:rdf="http://www.w3.org/1999/02/22-rdf-syntax-ns#"
  xmlns:rdfs="http://www.w3.org/2000/01/rdf-schema#"
  xmlns:owl="http://www.w3.org/2002/07/owl#"
  xmlns:xsd="http://www.w3.org/2001/XMLSchema#"
  xml:base="http://example.org/onto/">
  <owl:Class rdf:about="http://example.org/onto/class/google_cloud_run_service">
    <rdfs:label>google_cloud_run_service</rdfs:label>
    <rdfs:comment>#
#     ***     AUTO GENERATED CODE    ***    Type: MMv1     ***
#
# ----------------------------------------------------------------------------
#
#     This code is generated by Magic Modules using the following:
#
#     Configuration: https:#github.com/GoogleCloudPlatform/magic-modules/tree/main/mmv1/products/cloudrun/Service.yaml
#     Template:      https:#github.com/GoogleCloudPlatform/magic-modules/tree/main/mmv1/templates/terraform/resource.html.markdown.tmpl
#
#     DO NOT EDIT this file directly. Any changes made to this file will be
#     overwritten during the next generation cycle.
#
# ----------------------------------------------------------------------------
subcategory: "Cloud Run"
description: |-
  A Cloud Run service has a unique endpoint and autoscales containers.
---</rdfs:comment>
  </owl:Class>
  <owl:DatatypeProperty rdf:about="http://example.org/onto/prop/google_cloud_run_service_autogenerate_revision_name">
    <rdfs:label>autogenerate_revision_name</rdfs:label>
    <rdfs:comment>If set to 'true', the revision name (template.metadata.name) will be omitted and
autogenerated by Cloud Run. This cannot be set to 'true' while 'template.metadata.name'
is also set.
(For legacy support, if 'template.metadata.name' is unset in state while
this field is set to false, the revision name will still autogenerate.)</rdfs:comment>
    <rdfs:domain rdf:resource="http://example.org/onto/class/google_cloud_run_service"/>
    <rdfs:range rdf:resource="http://www.w3.org/2001/XMLSchema#string"/>
  </owl:DatatypeProperty>
  <owl:DatatypeProperty rdf:about="http://example.org/onto/prop/google_cloud_run_service_id">
    <rdfs:label>id</rdfs:label>
    <rdfs:domain rdf:resource="http://example.org/onto/class/google_cloud_run_service"/>
    <rdfs:range rdf:resource="http://www.w3.org/2001/XMLSchema#string"/>
  </owl:DatatypeProperty>
  <owl:DatatypeProperty rdf:about="http://example.org/onto/prop/google_cloud_run_service_location">
    <rdfs:label>location</rdfs:label>
    <rdfs:comment>The location of the cloud run instance. eg us-central1</rdfs:comment>
    <rdfs:domain rdf:resource="http://example.org/onto/class/google_cloud_run_service"/>
    <rdfs:range rdf:resource="http://www.w3.org/2001/XMLSchema#string"/>
  </owl:DatatypeProperty>
  <owl:DatatypeProperty rdf:about="http://example.org/onto/prop/google_cloud_run_service_name">
    <rdfs:label>name</rdfs:label>
    <rdfs:comment>Name must be unique within a Google Cloud project and region.
Is required when creating resources. Name is primarily intended
for creation idempotence and configuration definition. Cannot be updated.
More info: https://kubernetes.io/docs/concepts/overview/working-with-objects/names/#names</rdfs:comment>
    <rdfs:domain rdf:resource="http://example.org/onto/class/google_cloud_run_service"/>
    <rdfs:range rdf:resource="http://www.w3.org/2001/XMLSchema#string"/>
  </owl:DatatypeProperty>
  <owl:DatatypeProperty rdf:about="http://example.org/onto/prop/google_cloud_run_service_project">
    <rdfs:label>project</rdfs:label>
    <rdfs:domain rdf:resource="http://example.org/onto/class/google_cloud_run_service"/>
    <rdfs:range rdf:resource="http://www.w3.org/2001/XMLSchema#string"/>
  </owl:DatatypeProperty>
  <owl:DatatypeProperty rdf:about="http://example.org/onto/prop/google_cloud_run_service_status">
    <rdfs:label>status</rdfs:label>
    <rdfs:comment>The current status of the Service.</rdfs:comment>
    <rdfs:domain rdf:resource="http://example.org/onto/class/google_cloud_run_service"/>
    <rdfs:range rdf:resource="http://www.w3.org/2001/XMLSchema#string"/>
  </owl:DatatypeProperty>
  <owl:DatatypeProperty rdf:about="http://example.org/onto/prop/google_cloud_run_service_annotations">
    <rdfs:label>annotations</rdfs:label>
    <rdfs:comment>Annotations is a key value map stored with a resource that
may be set by external tools to store and retrieve arbitrary metadata.
More info: https://kubernetes.io/docs/concepts/overview/working-with-objects/annotations

**Note**: The Cloud Run API may add additional annotations that were not provided in your config.
If terraform plan shows a diff where a server-side annotation is added, you can add it to your config
or apply the lifecycle.ignore_changes rule to the metadata.0.annotations field.

Annotations with 'run.googleapis.com/' and 'autoscaling.knative.dev' are restricted. Use the following annotation
keys to configure features on a Service:

- 'run.googleapis.com/binary-authorization-breakglass' sets the [Binary Authorization breakglass](https://cloud.google.com/sdk/gcloud/reference/run/deploy#--breakglass).
- 'run.googleapis.com/binary-authorization' sets the [Binary Authorization](https://cloud.google.com/sdk/gcloud/reference/run/deploy#--binary-authorization).
- 'run.googleapis.com/client-name' sets the client name calling the Cloud Run API.
- 'run.googleapis.com/custom-audiences' sets the [custom audiences](https://cloud.google.com/sdk/gcloud/reference/alpha/run/deploy#--add-custom-audiences)
  that can be used in the audience field of ID token for authenticated requests.
- 'run.googleapis.com/description' sets a user defined description for the Service.
- 'run.googleapis.com/ingress' sets the [ingress settings](https://cloud.google.com/sdk/gcloud/reference/run/deploy#--ingress)
  for the Service. For example, '"run.googleapis.com/ingress" = "all"'.
- 'run.googleapis.com/launch-stage' sets the [launch stage](https://cloud.google.com/run/docs/troubleshooting#launch-stage-validation)
  when a preview feature is used. For example, '"run.googleapis.com/launch-stage": "BETA"'
- 'run.googleapis.com/minScale' sets the [minimum number of container instances](https://cloud.google.com/sdk/gcloud/reference/run/deploy#--min) of the Service.
- 'run.googleapis.com/scalingMode' sets the type of scaling mode for the service. The supported values for scaling mode are "manual" and "automatic". If not provided, it defaults to "automatic".
- 'run.googleapis.com/manualInstanceCount' sets the total instance count for the service in manual scaling mode. This number of instances is divided among all revisions with specified traffic based on the percent of traffic they are receiving.

**Note**: This field is non-authoritative, and will only manage the annotations present in your configuration.
Please refer to the field 'effective_annotations' for all of the annotations present on the resource.</rdfs:comment>
    <rdfs:domain rdf:resource="http://example.org/onto/class/google_cloud_run_service"/>
    <rdfs:range rdf:resource="http://www.w3.org/2001/XMLSchema#string"/>
  </owl:DatatypeProperty>
  <owl:DatatypeProperty rdf:about="http://example.org/onto/prop/google_cloud_run_service_effective_annotations">
    <rdfs:label>effective_annotations</rdfs:label>
    <rdfs:comment>All of annotations (key/value pairs) present on the resource in GCP, including the annotations configured through Terraform, other clients and services.</rdfs:comment>
    <rdfs:domain rdf:resource="http://example.org/onto/class/google_cloud_run_service"/>
    <rdfs:range rdf:resource="http://www.w3.org/2001/XMLSchema#string"/>
  </owl:DatatypeProperty>
  <owl:DatatypeProperty rdf:about="http://example.org/onto/prop/google_cloud_run_service_effective_labels">
    <rdfs:label>effective_labels</rdfs:label>
    <rdfs:comment>All of labels (key/value pairs) present on the resource in GCP, including the labels configured through Terraform, other clients and services.</rdfs:comment>
    <rdfs:domain rdf:resource="http://example.org/onto/class/google_cloud_run_service"/>
    <rdfs:range rdf:resource="http://www.w3.org/2001/XMLSchema#string"/>
  </owl:DatatypeProperty>
  <owl:DatatypeProperty rdf:about="http://example.org/onto/prop/google_cloud_run_service_generation">
    <rdfs:label>generation</rdfs:label>
    <rdfs:comment>A sequence number representing a specific generation of the desired state.</rdfs:comment>
    <rdfs:domain rdf:resource="http://example.org/onto/class/google_cloud_run_service"/>
    <rdfs:range rdf:resource="http://www.w3.org/2001/XMLSchema#string"/>
  </owl:DatatypeProperty>
  <owl:DatatypeProperty rdf:about="http://example.org/onto/prop/google_cloud_run_service_labels">
    <rdfs:label>labels</rdfs:label>
    <rdfs:comment>Map of string keys and values that can be used to organize and categorize
(scope and select) objects. May match selectors of replication controllers
and routes.

**Note**: This field is non-authoritative, and will only manage the labels present in your configuration.
Please refer to the field 'effective_labels' for all of the labels present on the resource.</rdfs:comment>
    <rdfs:domain rdf:resource="http://example.org/onto/class/google_cloud_run_service"/>
    <rdfs:range rdf:resource="http://www.w3.org/2001/XMLSchema#string"/>
  </owl:DatatypeProperty>
  <owl:DatatypeProperty rdf:about="http://example.org/onto/prop/google_cloud_run_service_namespace">
    <rdfs:label>namespace</rdfs:label>
    <rdfs:comment>In Cloud Run the namespace must be equal to either the
project ID or project number.</rdfs:comment>
    <rdfs:domain rdf:resource="http://example.org/onto/class/google_cloud_run_service"/>
    <rdfs:range rdf:resource="http://www.w3.org/2001/XMLSchema#string"/>
  </owl:DatatypeProperty>
  <owl:DatatypeProperty rdf:about="http://example.org/onto/prop/google_cloud_run_service_resource_version">
    <rdfs:label>resource_version</rdfs:label>
    <rdfs:comment>An opaque value that represents the internal version of this object that
can be used by clients to determine when objects have changed. May be used
for optimistic concurrency, change detection, and the watch operation on a
resource or set of resources. They may only be valid for a
particular resource or set of resources.</rdfs:comment>
    <rdfs:domain rdf:resource="http://example.org/onto/class/google_cloud_run_service"/>
    <rdfs:range rdf:resource="http://www.w3.org/2001/XMLSchema#string"/>
  </owl:DatatypeProperty>
  <owl:DatatypeProperty rdf:about="http://example.org/onto/prop/google_cloud_run_service_self_link">
    <rdfs:label>self_link</rdfs:label>
    <rdfs:comment>SelfLink is a URL representing this object.</rdfs:comment>
    <rdfs:domain rdf:resource="http://example.org/onto/class/google_cloud_run_service"/>
    <rdfs:range rdf:resource="http://www.w3.org/2001/XMLSchema#string"/>
  </owl:DatatypeProperty>
  <owl:DatatypeProperty rdf:about="http://example.org/onto/prop/google_cloud_run_service_terraform_labels">
    <rdfs:label>terraform_labels</rdfs:label>
    <rdfs:comment>The combination of labels configured directly on the resource
 and default labels configured on the provider.</rdfs:comment>
    <rdfs:domain rdf:resource="http://example.org/onto/class/google_cloud_run_service"/>
    <rdfs:range rdf:resource="http://www.w3.org/2001/XMLSchema#string"/>
  </owl:DatatypeProperty>
  <owl:DatatypeProperty rdf:about="http://example.org/onto/prop/google_cloud_run_service_uid">
    <rdfs:label>uid</rdfs:label>
    <rdfs:comment>UID is a unique id generated by the server on successful creation of a resource and is not
allowed to change on PUT operations.</rdfs:comment>
    <rdfs:domain rdf:resource="http://example.org/onto/class/google_cloud_run_service"/>
    <rdfs:range rdf:resource="http://www.w3.org/2001/XMLSchema#string"/>
  </owl:DatatypeProperty>
  <owl:DatatypeProperty rdf:about="http://example.org/onto/prop/google_cloud_run_service_annotations">
    <rdfs:label>annotations</rdfs:label>
    <rdfs:comment>Annotations is a key value map stored with a resource that
may be set by external tools to store and retrieve arbitrary metadata.
More info: https://kubernetes.io/docs/concepts/overview/working-with-objects/annotations

**Note**: The Cloud Run API may add additional annotations that were not provided in your config.
If terraform plan shows a diff where a server-side annotation is added, you can add it to your config
or apply the lifecycle.ignore_changes rule to the metadata.0.annotations field.

Annotations with 'run.googleapis.com/' and 'autoscaling.knative.dev' are restricted. Use the following annotation
keys to configure features on a Revision template:

- 'autoscaling.knative.dev/maxScale' sets the [maximum number of container
  instances](https://cloud.google.com/sdk/gcloud/reference/run/deploy#--max-instances) of the Revision to run.
- 'autoscaling.knative.dev/minScale' sets the [minimum number of container
  instances](https://cloud.google.com/sdk/gcloud/reference/run/deploy#--min-instances) of the Revision to run.
- 'run.googleapis.com/client-name' sets the client name calling the Cloud Run API.
- 'run.googleapis.com/cloudsql-instances' sets the [Cloud SQL
  instances](https://cloud.google.com/sdk/gcloud/reference/run/deploy#--add-cloudsql-instances) the Revision connects to.
- 'run.googleapis.com/cpu-throttling' sets whether to throttle the CPU when the container is not actively serving
  requests. See https://cloud.google.com/sdk/gcloud/reference/run/deploy#--[no-]cpu-throttling.
- 'run.googleapis.com/encryption-key-shutdown-hours' sets the number of hours to wait before an automatic shutdown
  server after CMEK key revocation is detected.
- 'run.googleapis.com/encryption-key' sets the [CMEK key](https://cloud.google.com/run/docs/securing/using-cmek)
  reference to encrypt the container with.
- 'run.googleapis.com/execution-environment' sets the [execution
  environment](https://cloud.google.com/sdk/gcloud/reference/run/deploy#--execution-environment)
  where the application will run.
- 'run.googleapis.com/post-key-revocation-action-type' sets the
  [action type](https://cloud.google.com/sdk/gcloud/reference/run/deploy#--post-key-revocation-action-type)
  after CMEK key revocation.
- 'run.googleapis.com/secrets' sets a list of key-value pairs to set as
  [secrets](https://cloud.google.com/run/docs/configuring/secrets#yaml).
- 'run.googleapis.com/sessionAffinity' sets whether to enable
  [session affinity](https://cloud.google.com/sdk/gcloud/reference/beta/run/deploy#--[no-]session-affinity)
  for connections to the Revision.
- 'run.googleapis.com/startup-cpu-boost' sets whether to allocate extra CPU to containers on startup.
  See https://cloud.google.com/sdk/gcloud/reference/run/deploy#--[no-]cpu-boost.
- 'run.googleapis.com/network-interfaces' sets [Direct VPC egress](https://cloud.google.com/run/docs/configuring/vpc-direct-vpc#yaml)
  for the Revision.
- 'run.googleapis.com/vpc-access-connector' sets a [VPC connector](https://cloud.google.com/run/docs/configuring/connecting-vpc#terraform_1)
  for the Revision.
- 'run.googleapis.com/vpc-access-egress' sets the outbound traffic to send through the VPC connector for this resource.
  See https://cloud.google.com/sdk/gcloud/reference/run/deploy#--vpc-egress.
- 'run.googleapis.com/gpu-zonal-redundancy-disabled' sets
  [GPU zonal redundancy](https://cloud.google.com/run/docs/configuring/services/gpu-zonal-redundancy) for the Revision.
- 'run.googleapis.com/health-check-disabled' disabled health checking containers during deployment.</rdfs:comment>
    <rdfs:domain rdf:resource="http://example.org/onto/class/google_cloud_run_service"/>
    <rdfs:range rdf:resource="http://www.w3.org/2001/XMLSchema#string"/>
  </owl:DatatypeProperty>
  <owl:DatatypeProperty rdf:about="http://example.org/onto/prop/google_cloud_run_service_generation">
    <rdfs:label>generation</rdfs:label>
    <rdfs:comment>A sequence number representing a specific generation of the desired state.</rdfs:comment>
    <rdfs:domain rdf:resource="http://example.org/onto/class/google_cloud_run_service"/>
    <rdfs:range rdf:resource="http://www.w3.org/2001/XMLSchema#string"/>
  </owl:DatatypeProperty>
  <owl:DatatypeProperty rdf:about="http://example.org/onto/prop/google_cloud_run_service_labels">
    <rdfs:label>labels</rdfs:label>
    <rdfs:comment>Map of string keys and values that can be used to organize and categorize
(scope and select) objects.</rdfs:comment>
    <rdfs:domain rdf:resource="http://example.org/onto/class/google_cloud_run_service"/>
    <rdfs:range rdf:resource="http://www.w3.org/2001/XMLSchema#string"/>
  </owl:DatatypeProperty>
  <owl:DatatypeProperty rdf:about="http://example.org/onto/prop/google_cloud_run_service_name">
    <rdfs:label>name</rdfs:label>
    <rdfs:comment>Name must be unique within a Google Cloud project and region.
Is required when creating resources. Name is primarily intended
for creation idempotence and configuration definition. Cannot be updated.</rdfs:comment>
    <rdfs:domain rdf:resource="http://example.org/onto/class/google_cloud_run_service"/>
    <rdfs:range rdf:resource="http://www.w3.org/2001/XMLSchema#string"/>
  </owl:DatatypeProperty>
  <owl:DatatypeProperty rdf:about="http://example.org/onto/prop/google_cloud_run_service_namespace">
    <rdfs:label>namespace</rdfs:label>
    <rdfs:comment>In Cloud Run the namespace must be equal to either the
project ID or project number. It will default to the resource's project.</rdfs:comment>
    <rdfs:domain rdf:resource="http://example.org/onto/class/google_cloud_run_service"/>
    <rdfs:range rdf:resource="http://www.w3.org/2001/XMLSchema#string"/>
  </owl:DatatypeProperty>
  <owl:DatatypeProperty rdf:about="http://example.org/onto/prop/google_cloud_run_service_resource_version">
    <rdfs:label>resource_version</rdfs:label>
    <rdfs:comment>An opaque value that represents the internal version of this object that
can be used by clients to determine when objects have changed. May be used
for optimistic concurrency, change detection, and the watch operation on a
resource or set of resources. They may only be valid for a
particular resource or set of resources.</rdfs:comment>
    <rdfs:domain rdf:resource="http://example.org/onto/class/google_cloud_run_service"/>
    <rdfs:range rdf:resource="http://www.w3.org/2001/XMLSchema#string"/>
  </owl:DatatypeProperty>
  <owl:DatatypeProperty rdf:about="http://example.org/onto/prop/google_cloud_run_service_self_link">
    <rdfs:label>self_link</rdfs:label>
    <rdfs:comment>SelfLink is a URL representing this object.</rdfs:comment>
    <rdfs:domain rdf:resource="http://example.org/onto/class/google_cloud_run_service"/>
    <rdfs:range rdf:resource="http://www.w3.org/2001/XMLSchema#string"/>
  </owl:DatatypeProperty>
  <owl:DatatypeProperty rdf:about="http://example.org/onto/prop/google_cloud_run_service_uid">
    <rdfs:label>uid</rdfs:label>
    <rdfs:comment>UID is a unique id generated by the server on successful creation of a resource and is not
allowed to change on PUT operations.</rdfs:comment>
    <rdfs:domain rdf:resource="http://example.org/onto/class/google_cloud_run_service"/>
    <rdfs:range rdf:resource="http://www.w3.org/2001/XMLSchema#string"/>
  </owl:DatatypeProperty>
  <owl:DatatypeProperty rdf:about="http://example.org/onto/prop/google_cloud_run_service_container_concurrency">
    <rdfs:label>container_concurrency</rdfs:label>
    <rdfs:comment>ContainerConcurrency specifies the maximum allowed in-flight (concurrent)
requests per container of the Revision. If not specified or 0, defaults to 80 when
requested CPU >= 1 and defaults to 1 when requested CPU < 1.</rdfs:comment>
    <rdfs:domain rdf:resource="http://example.org/onto/class/google_cloud_run_service"/>
    <rdfs:range rdf:resource="http://www.w3.org/2001/XMLSchema#string"/>
  </owl:DatatypeProperty>
  <owl:DatatypeProperty rdf:about="http://example.org/onto/prop/google_cloud_run_service_node_selector">
    <rdfs:label>node_selector</rdfs:label>
    <rdfs:comment>Node Selector describes the hardware requirements of the resources.
Use the following node selector keys to configure features on a Revision:
  - 'run.googleapis.com/accelerator' sets the [type of GPU](https://cloud.google.com/run/docs/configuring/services/gpu) required by the Revision to run.</rdfs:comment>
    <rdfs:domain rdf:resource="http://example.org/onto/class/google_cloud_run_service"/>
    <rdfs:range rdf:resource="http://www.w3.org/2001/XMLSchema#string"/>
  </owl:DatatypeProperty>
  <owl:DatatypeProperty rdf:about="http://example.org/onto/prop/google_cloud_run_service_service_account_name">
    <rdfs:label>service_account_name</rdfs:label>
    <rdfs:comment>Email address of the IAM service account associated with the revision of the
service. The service account represents the identity of the running revision,
and determines what permissions the revision has. If not provided, the revision
will use the project's default service account.</rdfs:comment>
    <rdfs:domain rdf:resource="http://example.org/onto/class/google_cloud_run_service"/>
    <rdfs:range rdf:resource="http://www.w3.org/2001/XMLSchema#string"/>
  </owl:DatatypeProperty>
  <owl:DatatypeProperty rdf:about="http://example.org/onto/prop/google_cloud_run_service_serving_state">
    <rdfs:label>serving_state</rdfs:label>
    <rdfs:comment>ServingState holds a value describing the state the resources
are in for this Revision.
It is expected
that the system will manipulate this based on routability and load.</rdfs:comment>
    <rdfs:domain rdf:resource="http://example.org/onto/class/google_cloud_run_service"/>
    <rdfs:range rdf:resource="http://www.w3.org/2001/XMLSchema#string"/>
  </owl:DatatypeProperty>
  <owl:DatatypeProperty rdf:about="http://example.org/onto/prop/google_cloud_run_service_timeout_seconds">
    <rdfs:label>timeout_seconds</rdfs:label>
    <rdfs:comment>TimeoutSeconds holds the max duration the instance is allowed for responding to a request.</rdfs:comment>
    <rdfs:domain rdf:resource="http://example.org/onto/class/google_cloud_run_service"/>
    <rdfs:range rdf:resource="http://www.w3.org/2001/XMLSchema#string"/>
  </owl:DatatypeProperty>
  <owl:DatatypeProperty rdf:about="http://example.org/onto/prop/google_cloud_run_service_args">
    <rdfs:label>args</rdfs:label>
    <rdfs:comment>Arguments to the entrypoint.
The docker image's CMD is used if this is not provided.</rdfs:comment>
    <rdfs:domain rdf:resource="http://example.org/onto/class/google_cloud_run_service"/>
    <rdfs:range rdf:resource="http://www.w3.org/2001/XMLSchema#string"/>
  </owl:DatatypeProperty>
  <owl:DatatypeProperty rdf:about="http://example.org/onto/prop/google_cloud_run_service_command">
    <rdfs:label>command</rdfs:label>
    <rdfs:comment>Entrypoint array. Not executed within a shell.
The docker image's ENTRYPOINT is used if this is not provided.</rdfs:comment>
    <rdfs:domain rdf:resource="http://example.org/onto/class/google_cloud_run_service"/>
    <rdfs:range rdf:resource="http://www.w3.org/2001/XMLSchema#string"/>
  </owl:DatatypeProperty>
  <owl:DatatypeProperty rdf:about="http://example.org/onto/prop/google_cloud_run_service_image">
    <rdfs:label>image</rdfs:label>
    <rdfs:comment>Docker image name. This is most often a reference to a container located
in the container registry, such as gcr.io/cloudrun/hello</rdfs:comment>
    <rdfs:domain rdf:resource="http://example.org/onto/class/google_cloud_run_service"/>
    <rdfs:range rdf:resource="http://www.w3.org/2001/XMLSchema#string"/>
  </owl:DatatypeProperty>
  <owl:DatatypeProperty rdf:about="http://example.org/onto/prop/google_cloud_run_service_name">
    <rdfs:label>name</rdfs:label>
    <rdfs:comment>Name of the container</rdfs:comment>
    <rdfs:domain rdf:resource="http://example.org/onto/class/google_cloud_run_service"/>
    <rdfs:range rdf:resource="http://www.w3.org/2001/XMLSchema#string"/>
  </owl:DatatypeProperty>
  <owl:DatatypeProperty rdf:about="http://example.org/onto/prop/google_cloud_run_service_working_dir">
    <rdfs:label>working_dir</rdfs:label>
    <rdfs:comment>Container's working directory.
If not specified, the container runtime's default will be used, which
might be configured in the container image.</rdfs:comment>
    <rdfs:domain rdf:resource="http://example.org/onto/class/google_cloud_run_service"/>
    <rdfs:range rdf:resource="http://www.w3.org/2001/XMLSchema#string"/>
  </owl:DatatypeProperty>
  <owl:DatatypeProperty rdf:about="http://example.org/onto/prop/google_cloud_run_service_name">
    <rdfs:label>name</rdfs:label>
    <rdfs:comment>Name of the environment variable.</rdfs:comment>
    <rdfs:domain rdf:resource="http://example.org/onto/class/google_cloud_run_service"/>
    <rdfs:range rdf:resource="http://www.w3.org/2001/XMLSchema#string"/>
  </owl:DatatypeProperty>
  <owl:DatatypeProperty rdf:about="http://example.org/onto/prop/google_cloud_run_service_value">
    <rdfs:label>value</rdfs:label>
    <rdfs:comment>Defaults to "".</rdfs:comment>
    <rdfs:domain rdf:resource="http://example.org/onto/class/google_cloud_run_service"/>
    <rdfs:range rdf:resource="http://www.w3.org/2001/XMLSchema#string"/>
  </owl:DatatypeProperty>
  <owl:DatatypeProperty rdf:about="http://example.org/onto/prop/google_cloud_run_service_key">
    <rdfs:label>key</rdfs:label>
    <rdfs:comment>A Cloud Secret Manager secret version. Must be 'latest' for the latest
version or an integer for a specific version.</rdfs:comment>
    <rdfs:domain rdf:resource="http://example.org/onto/class/google_cloud_run_service"/>
    <rdfs:range rdf:resource="http://www.w3.org/2001/XMLSchema#string"/>
  </owl:DatatypeProperty>
  <owl:DatatypeProperty rdf:about="http://example.org/onto/prop/google_cloud_run_service_name">
    <rdfs:label>name</rdfs:label>
    <rdfs:comment>The name of the secret in Cloud Secret Manager. By default, the secret is assumed to be in the same project.
If the secret is in another project, you must define an alias.
An alias definition has the form:
{alias}:projects/{project-id|project-number}/secrets/{secret-name}.
If multiple alias definitions are needed, they must be separated by commas.
The alias definitions must be set on the run.googleapis.com/secrets annotation.</rdfs:comment>
    <rdfs:domain rdf:resource="http://example.org/onto/class/google_cloud_run_service"/>
    <rdfs:range rdf:resource="http://www.w3.org/2001/XMLSchema#string"/>
  </owl:DatatypeProperty>
  <owl:DatatypeProperty rdf:about="http://example.org/onto/prop/google_cloud_run_service_prefix">
    <rdfs:label>prefix</rdfs:label>
    <rdfs:comment>An optional identifier to prepend to each key in the ConfigMap.</rdfs:comment>
    <rdfs:domain rdf:resource="http://example.org/onto/class/google_cloud_run_service"/>
    <rdfs:range rdf:resource="http://www.w3.org/2001/XMLSchema#string"/>
  </owl:DatatypeProperty>
  <owl:DatatypeProperty rdf:about="http://example.org/onto/prop/google_cloud_run_service_optional">
    <rdfs:label>optional</rdfs:label>
    <rdfs:comment>Specify whether the ConfigMap must be defined</rdfs:comment>
    <rdfs:domain rdf:resource="http://example.org/onto/class/google_cloud_run_service"/>
    <rdfs:range rdf:resource="http://www.w3.org/2001/XMLSchema#string"/>
  </owl:DatatypeProperty>
  <owl:DatatypeProperty rdf:about="http://example.org/onto/prop/google_cloud_run_service_name">
    <rdfs:label>name</rdfs:label>
    <rdfs:comment>Name of the referent.</rdfs:comment>
    <rdfs:domain rdf:resource="http://example.org/onto/class/google_cloud_run_service"/>
    <rdfs:range rdf:resource="http://www.w3.org/2001/XMLSchema#string"/>
  </owl:DatatypeProperty>
  <owl:DatatypeProperty rdf:about="http://example.org/onto/prop/google_cloud_run_service_optional">
    <rdfs:label>optional</rdfs:label>
    <rdfs:comment>Specify whether the Secret must be defined</rdfs:comment>
    <rdfs:domain rdf:resource="http://example.org/onto/class/google_cloud_run_service"/>
    <rdfs:range rdf:resource="http://www.w3.org/2001/XMLSchema#string"/>
  </owl:DatatypeProperty>
  <owl:DatatypeProperty rdf:about="http://example.org/onto/prop/google_cloud_run_service_name">
    <rdfs:label>name</rdfs:label>
    <rdfs:comment>Name of the referent.</rdfs:comment>
    <rdfs:domain rdf:resource="http://example.org/onto/class/google_cloud_run_service"/>
    <rdfs:range rdf:resource="http://www.w3.org/2001/XMLSchema#string"/>
  </owl:DatatypeProperty>
  <owl:DatatypeProperty rdf:about="http://example.org/onto/prop/google_cloud_run_service_failure_threshold">
    <rdfs:label>failure_threshold</rdfs:label>
    <rdfs:comment>Minimum consecutive failures for the probe to be considered failed after
having succeeded. Defaults to 3. Minimum value is 1.</rdfs:comment>
    <rdfs:domain rdf:resource="http://example.org/onto/class/google_cloud_run_service"/>
    <rdfs:range rdf:resource="http://www.w3.org/2001/XMLSchema#string"/>
  </owl:DatatypeProperty>
  <owl:DatatypeProperty rdf:about="http://example.org/onto/prop/google_cloud_run_service_initial_delay_seconds">
    <rdfs:label>initial_delay_seconds</rdfs:label>
    <rdfs:comment>Number of seconds after the container has started before the probe is
initiated.
Defaults to 0 seconds. Minimum value is 0. Maximum value is 3600.</rdfs:comment>
    <rdfs:domain rdf:resource="http://example.org/onto/class/google_cloud_run_service"/>
    <rdfs:range rdf:resource="http://www.w3.org/2001/XMLSchema#string"/>
  </owl:DatatypeProperty>
  <owl:DatatypeProperty rdf:about="http://example.org/onto/prop/google_cloud_run_service_period_seconds">
    <rdfs:label>period_seconds</rdfs:label>
    <rdfs:comment>How often (in seconds) to perform the probe.
Default to 10 seconds. Minimum value is 1. Maximum value is 3600.</rdfs:comment>
    <rdfs:domain rdf:resource="http://example.org/onto/class/google_cloud_run_service"/>
    <rdfs:range rdf:resource="http://www.w3.org/2001/XMLSchema#string"/>
  </owl:DatatypeProperty>
  <owl:DatatypeProperty rdf:about="http://example.org/onto/prop/google_cloud_run_service_timeout_seconds">
    <rdfs:label>timeout_seconds</rdfs:label>
    <rdfs:comment>Number of seconds after which the probe times out.
Defaults to 1 second. Minimum value is 1. Maximum value is 3600.
Must be smaller than period_seconds.</rdfs:comment>
    <rdfs:domain rdf:resource="http://example.org/onto/class/google_cloud_run_service"/>
    <rdfs:range rdf:resource="http://www.w3.org/2001/XMLSchema#string"/>
  </owl:DatatypeProperty>
  <owl:DatatypeProperty rdf:about="http://example.org/onto/prop/google_cloud_run_service_port">
    <rdfs:label>port</rdfs:label>
    <rdfs:comment>Port number to access on the container. Number must be in the range 1 to 65535.
If not specified, defaults to the same value as container.ports[0].containerPort.</rdfs:comment>
    <rdfs:domain rdf:resource="http://example.org/onto/class/google_cloud_run_service"/>
    <rdfs:range rdf:resource="http://www.w3.org/2001/XMLSchema#string"/>
  </owl:DatatypeProperty>
  <owl:DatatypeProperty rdf:about="http://example.org/onto/prop/google_cloud_run_service_service">
    <rdfs:label>service</rdfs:label>
    <rdfs:comment>The name of the service to place in the gRPC HealthCheckRequest
(see https://github.com/grpc/grpc/blob/master/doc/health-checking.md).
If this is not specified, the default behavior is defined by gRPC.</rdfs:comment>
    <rdfs:domain rdf:resource="http://example.org/onto/class/google_cloud_run_service"/>
    <rdfs:range rdf:resource="http://www.w3.org/2001/XMLSchema#string"/>
  </owl:DatatypeProperty>
  <owl:DatatypeProperty rdf:about="http://example.org/onto/prop/google_cloud_run_service_path">
    <rdfs:label>path</rdfs:label>
    <rdfs:comment>Path to access on the HTTP server. If set, it should not be empty string.</rdfs:comment>
    <rdfs:domain rdf:resource="http://example.org/onto/class/google_cloud_run_service"/>
    <rdfs:range rdf:resource="http://www.w3.org/2001/XMLSchema#string"/>
  </owl:DatatypeProperty>
  <owl:DatatypeProperty rdf:about="http://example.org/onto/prop/google_cloud_run_service_port">
    <rdfs:label>port</rdfs:label>
    <rdfs:comment>Port number to access on the container. Number must be in the range 1 to 65535.
If not specified, defaults to the same value as container.ports[0].containerPort.</rdfs:comment>
    <rdfs:domain rdf:resource="http://example.org/onto/class/google_cloud_run_service"/>
    <rdfs:range rdf:resource="http://www.w3.org/2001/XMLSchema#string"/>
  </owl:DatatypeProperty>
  <owl:DatatypeProperty rdf:about="http://example.org/onto/prop/google_cloud_run_service_name">
    <rdfs:label>name</rdfs:label>
    <rdfs:comment>The header field name.</rdfs:comment>
    <rdfs:domain rdf:resource="http://example.org/onto/class/google_cloud_run_service"/>
    <rdfs:range rdf:resource="http://www.w3.org/2001/XMLSchema#string"/>
  </owl:DatatypeProperty>
  <owl:DatatypeProperty rdf:about="http://example.org/onto/prop/google_cloud_run_service_value">
    <rdfs:label>value</rdfs:label>
    <rdfs:comment>The header field value.</rdfs:comment>
    <rdfs:domain rdf:resource="http://example.org/onto/class/google_cloud_run_service"/>
    <rdfs:range rdf:resource="http://www.w3.org/2001/XMLSchema#string"/>
  </owl:DatatypeProperty>
  <owl:DatatypeProperty rdf:about="http://example.org/onto/prop/google_cloud_run_service_container_port">
    <rdfs:label>container_port</rdfs:label>
    <rdfs:comment>Port number the container listens on. This must be a valid port number (between 1 and 65535). Defaults to "8080".</rdfs:comment>
    <rdfs:domain rdf:resource="http://example.org/onto/class/google_cloud_run_service"/>
    <rdfs:range rdf:resource="http://www.w3.org/2001/XMLSchema#string"/>
  </owl:DatatypeProperty>
  <owl:DatatypeProperty rdf:about="http://example.org/onto/prop/google_cloud_run_service_name">
    <rdfs:label>name</rdfs:label>
    <rdfs:comment>If specified, used to specify which protocol to use. Allowed values are "http1" (HTTP/1) and "h2c" (HTTP/2 end-to-end). Defaults to "http1".</rdfs:comment>
    <rdfs:domain rdf:resource="http://example.org/onto/class/google_cloud_run_service"/>
    <rdfs:range rdf:resource="http://www.w3.org/2001/XMLSchema#string"/>
  </owl:DatatypeProperty>
  <owl:DatatypeProperty rdf:about="http://example.org/onto/prop/google_cloud_run_service_protocol">
    <rdfs:label>protocol</rdfs:label>
    <rdfs:comment>Protocol for port. Must be "TCP". Defaults to "TCP".</rdfs:comment>
    <rdfs:domain rdf:resource="http://example.org/onto/class/google_cloud_run_service"/>
    <rdfs:range rdf:resource="http://www.w3.org/2001/XMLSchema#string"/>
  </owl:DatatypeProperty>
  <owl:DatatypeProperty rdf:about="http://example.org/onto/prop/google_cloud_run_service_limits">
    <rdfs:label>limits</rdfs:label>
    <rdfs:comment>Limits describes the maximum amount of compute resources allowed.
The values of the map is string form of the 'quantity' k8s type:
https://github.com/kubernetes/kubernetes/blob/master/staging/src/k8s.io/apimachinery/pkg/api/resource/quantity.go</rdfs:comment>
    <rdfs:domain rdf:resource="http://example.org/onto/class/google_cloud_run_service"/>
    <rdfs:range rdf:resource="http://www.w3.org/2001/XMLSchema#string"/>
  </owl:DatatypeProperty>
  <owl:DatatypeProperty rdf:about="http://example.org/onto/prop/google_cloud_run_service_requests">
    <rdfs:label>requests</rdfs:label>
    <rdfs:comment>Requests describes the minimum amount of compute resources required.
If Requests is omitted for a container, it defaults to Limits if that is
explicitly specified, otherwise to an implementation-defined value.
The values of the map is string form of the 'quantity' k8s type:
https://github.com/kubernetes/kubernetes/blob/master/staging/src/k8s.io/apimachinery/pkg/api/resource/quantity.go</rdfs:comment>
    <rdfs:domain rdf:resource="http://example.org/onto/class/google_cloud_run_service"/>
    <rdfs:range rdf:resource="http://www.w3.org/2001/XMLSchema#string"/>
  </owl:DatatypeProperty>
  <owl:DatatypeProperty rdf:about="http://example.org/onto/prop/google_cloud_run_service_failure_threshold">
    <rdfs:label>failure_threshold</rdfs:label>
    <rdfs:comment>Minimum consecutive failures for the probe to be considered failed after
having succeeded. Defaults to 3. Minimum value is 1.</rdfs:comment>
    <rdfs:domain rdf:resource="http://example.org/onto/class/google_cloud_run_service"/>
    <rdfs:range rdf:resource="http://www.w3.org/2001/XMLSchema#string"/>
  </owl:DatatypeProperty>
  <owl:DatatypeProperty rdf:about="http://example.org/onto/prop/google_cloud_run_service_initial_delay_seconds">
    <rdfs:label>initial_delay_seconds</rdfs:label>
    <rdfs:comment>Number of seconds after the container has started before the probe is
initiated.
Defaults to 0 seconds. Minimum value is 0. Maximum value is 240.</rdfs:comment>
    <rdfs:domain rdf:resource="http://example.org/onto/class/google_cloud_run_service"/>
    <rdfs:range rdf:resource="http://www.w3.org/2001/XMLSchema#string"/>
  </owl:DatatypeProperty>
  <owl:DatatypeProperty rdf:about="http://example.org/onto/prop/google_cloud_run_service_period_seconds">
    <rdfs:label>period_seconds</rdfs:label>
    <rdfs:comment>How often (in seconds) to perform the probe.
Default to 10 seconds. Minimum value is 1. Maximum value is 240.</rdfs:comment>
    <rdfs:domain rdf:resource="http://example.org/onto/class/google_cloud_run_service"/>
    <rdfs:range rdf:resource="http://www.w3.org/2001/XMLSchema#string"/>
  </owl:DatatypeProperty>
  <owl:DatatypeProperty rdf:about="http://example.org/onto/prop/google_cloud_run_service_timeout_seconds">
    <rdfs:label>timeout_seconds</rdfs:label>
    <rdfs:comment>Number of seconds after which the probe times out.
Defaults to 1 second. Minimum value is 1. Maximum value is 3600.
Must be smaller than periodSeconds.</rdfs:comment>
    <rdfs:domain rdf:resource="http://example.org/onto/class/google_cloud_run_service"/>
    <rdfs:range rdf:resource="http://www.w3.org/2001/XMLSchema#string"/>
  </owl:DatatypeProperty>
  <owl:DatatypeProperty rdf:about="http://example.org/onto/prop/google_cloud_run_service_port">
    <rdfs:label>port</rdfs:label>
    <rdfs:comment>Port number to access on the container. Number must be in the range 1 to 65535.
If not specified, defaults to the same value as container.ports[0].containerPort.</rdfs:comment>
    <rdfs:domain rdf:resource="http://example.org/onto/class/google_cloud_run_service"/>
    <rdfs:range rdf:resource="http://www.w3.org/2001/XMLSchema#string"/>
  </owl:DatatypeProperty>
  <owl:DatatypeProperty rdf:about="http://example.org/onto/prop/google_cloud_run_service_service">
    <rdfs:label>service</rdfs:label>
    <rdfs:comment>The name of the service to place in the gRPC HealthCheckRequest
(see https://github.com/grpc/grpc/blob/master/doc/health-checking.md).
If this is not specified, the default behavior is defined by gRPC.</rdfs:comment>
    <rdfs:domain rdf:resource="http://example.org/onto/class/google_cloud_run_service"/>
    <rdfs:range rdf:resource="http://www.w3.org/2001/XMLSchema#string"/>
  </owl:DatatypeProperty>
  <owl:DatatypeProperty rdf:about="http://example.org/onto/prop/google_cloud_run_service_path">
    <rdfs:label>path</rdfs:label>
    <rdfs:comment>Path to access on the HTTP server. If set, it should not be empty string.</rdfs:comment>
    <rdfs:domain rdf:resource="http://example.org/onto/class/google_cloud_run_service"/>
    <rdfs:range rdf:resource="http://www.w3.org/2001/XMLSchema#string"/>
  </owl:DatatypeProperty>
  <owl:DatatypeProperty rdf:about="http://example.org/onto/prop/google_cloud_run_service_port">
    <rdfs:label>port</rdfs:label>
    <rdfs:comment>Port number to access on the container. Number must be in the range 1 to 65535.
If not specified, defaults to the same value as container.ports[0].containerPort.</rdfs:comment>
    <rdfs:domain rdf:resource="http://example.org/onto/class/google_cloud_run_service"/>
    <rdfs:range rdf:resource="http://www.w3.org/2001/XMLSchema#string"/>
  </owl:DatatypeProperty>
  <owl:DatatypeProperty rdf:about="http://example.org/onto/prop/google_cloud_run_service_name">
    <rdfs:label>name</rdfs:label>
    <rdfs:comment>The header field name.</rdfs:comment>
    <rdfs:domain rdf:resource="http://example.org/onto/class/google_cloud_run_service"/>
    <rdfs:range rdf:resource="http://www.w3.org/2001/XMLSchema#string"/>
  </owl:DatatypeProperty>
  <owl:DatatypeProperty rdf:about="http://example.org/onto/prop/google_cloud_run_service_value">
    <rdfs:label>value</rdfs:label>
    <rdfs:comment>The header field value.</rdfs:comment>
    <rdfs:domain rdf:resource="http://example.org/onto/class/google_cloud_run_service"/>
    <rdfs:range rdf:resource="http://www.w3.org/2001/XMLSchema#string"/>
  </owl:DatatypeProperty>
  <owl:DatatypeProperty rdf:about="http://example.org/onto/prop/google_cloud_run_service_port">
    <rdfs:label>port</rdfs:label>
    <rdfs:comment>Port number to access on the container. Number must be in the range 1 to 65535.
If not specified, defaults to the same value as container.ports[0].containerPort.</rdfs:comment>
    <rdfs:domain rdf:resource="http://example.org/onto/class/google_cloud_run_service"/>
    <rdfs:range rdf:resource="http://www.w3.org/2001/XMLSchema#string"/>
  </owl:DatatypeProperty>
  <owl:DatatypeProperty rdf:about="http://example.org/onto/prop/google_cloud_run_service_mount_path">
    <rdfs:label>mount_path</rdfs:label>
    <rdfs:comment>Path within the container at which the volume should be mounted.  Must
not contain ':'.</rdfs:comment>
    <rdfs:domain rdf:resource="http://example.org/onto/class/google_cloud_run_service"/>
    <rdfs:range rdf:resource="http://www.w3.org/2001/XMLSchema#string"/>
  </owl:DatatypeProperty>
  <owl:DatatypeProperty rdf:about="http://example.org/onto/prop/google_cloud_run_service_name">
    <rdfs:label>name</rdfs:label>
    <rdfs:comment>This must match the Name of a Volume.</rdfs:comment>
    <rdfs:domain rdf:resource="http://example.org/onto/class/google_cloud_run_service"/>
    <rdfs:range rdf:resource="http://www.w3.org/2001/XMLSchema#string"/>
  </owl:DatatypeProperty>
  <owl:DatatypeProperty rdf:about="http://example.org/onto/prop/google_cloud_run_service_sub_path">
    <rdfs:label>sub_path</rdfs:label>
    <rdfs:comment>Path within the volume from which the container's volume should be mounted.</rdfs:comment>
    <rdfs:domain rdf:resource="http://example.org/onto/class/google_cloud_run_service"/>
    <rdfs:range rdf:resource="http://www.w3.org/2001/XMLSchema#string"/>
  </owl:DatatypeProperty>
  <owl:DatatypeProperty rdf:about="http://example.org/onto/prop/google_cloud_run_service_name">
    <rdfs:label>name</rdfs:label>
    <rdfs:comment>Volume's name.</rdfs:comment>
    <rdfs:domain rdf:resource="http://example.org/onto/class/google_cloud_run_service"/>
    <rdfs:range rdf:resource="http://www.w3.org/2001/XMLSchema#string"/>
  </owl:DatatypeProperty>
  <owl:DatatypeProperty rdf:about="http://example.org/onto/prop/google_cloud_run_service_driver">
    <rdfs:label>driver</rdfs:label>
    <rdfs:comment>Unique name representing the type of file system to be created. Cloud Run supports the following values:
  * gcsfuse.run.googleapis.com: Mount a Google Cloud Storage bucket using GCSFuse. This driver requires the
    run.googleapis.com/execution-environment annotation to be unset or set to "gen2"</rdfs:comment>
    <rdfs:domain rdf:resource="http://example.org/onto/class/google_cloud_run_service"/>
    <rdfs:range rdf:resource="http://www.w3.org/2001/XMLSchema#string"/>
  </owl:DatatypeProperty>
  <owl:DatatypeProperty rdf:about="http://example.org/onto/prop/google_cloud_run_service_read_only">
    <rdfs:label>read_only</rdfs:label>
    <rdfs:comment>If true, all mounts created from this volume will be read-only.</rdfs:comment>
    <rdfs:domain rdf:resource="http://example.org/onto/class/google_cloud_run_service"/>
    <rdfs:range rdf:resource="http://www.w3.org/2001/XMLSchema#string"/>
  </owl:DatatypeProperty>
  <owl:DatatypeProperty rdf:about="http://example.org/onto/prop/google_cloud_run_service_volume_attributes">
    <rdfs:label>volume_attributes</rdfs:label>
    <rdfs:comment>Driver-specific attributes. The following options are supported for available drivers:
  * gcsfuse.run.googleapis.com
    * bucketName: The name of the Cloud Storage Bucket that backs this volume. The Cloud Run Service identity must have access to this bucket.</rdfs:comment>
    <rdfs:domain rdf:resource="http://example.org/onto/class/google_cloud_run_service"/>
    <rdfs:range rdf:resource="http://www.w3.org/2001/XMLSchema#string"/>
  </owl:DatatypeProperty>
  <owl:DatatypeProperty rdf:about="http://example.org/onto/prop/google_cloud_run_service_medium">
    <rdfs:label>medium</rdfs:label>
    <rdfs:comment>The medium on which the data is stored. The default is "" which means to use the node's default medium. Must be an empty string (default) or Memory.</rdfs:comment>
    <rdfs:domain rdf:resource="http://example.org/onto/class/google_cloud_run_service"/>
    <rdfs:range rdf:resource="http://www.w3.org/2001/XMLSchema#string"/>
  </owl:DatatypeProperty>
  <owl:DatatypeProperty rdf:about="http://example.org/onto/prop/google_cloud_run_service_size_limit">
    <rdfs:label>size_limit</rdfs:label>
    <rdfs:comment>Limit on the storage usable by this EmptyDir volume. The size limit is also applicable for memory medium. The maximum usage on memory medium EmptyDir would be the minimum value between the SizeLimit specified here and the sum of memory limits of all containers in a pod. This field's values are of the 'Quantity' k8s type: https://kubernetes.io/docs/reference/kubernetes-api/common-definitions/quantity/. The default is nil which means that the limit is undefined. More info: https://kubernetes.io/docs/concepts/storage/volumes/#emptydir.</rdfs:comment>
    <rdfs:domain rdf:resource="http://example.org/onto/class/google_cloud_run_service"/>
    <rdfs:range rdf:resource="http://www.w3.org/2001/XMLSchema#string"/>
  </owl:DatatypeProperty>
  <owl:DatatypeProperty rdf:about="http://example.org/onto/prop/google_cloud_run_service_path">
    <rdfs:label>path</rdfs:label>
    <rdfs:comment>Path exported by the NFS server</rdfs:comment>
    <rdfs:domain rdf:resource="http://example.org/onto/class/google_cloud_run_service"/>
    <rdfs:range rdf:resource="http://www.w3.org/2001/XMLSchema#string"/>
  </owl:DatatypeProperty>
  <owl:DatatypeProperty rdf:about="http://example.org/onto/prop/google_cloud_run_service_read_only">
    <rdfs:label>read_only</rdfs:label>
    <rdfs:comment>If true, mount the NFS volume as read only in all mounts. Defaults to false.</rdfs:comment>
    <rdfs:domain rdf:resource="http://example.org/onto/class/google_cloud_run_service"/>
    <rdfs:range rdf:resource="http://www.w3.org/2001/XMLSchema#string"/>
  </owl:DatatypeProperty>
  <owl:DatatypeProperty rdf:about="http://example.org/onto/prop/google_cloud_run_service_server">
    <rdfs:label>server</rdfs:label>
    <rdfs:comment>IP address or hostname of the NFS server</rdfs:comment>
    <rdfs:domain rdf:resource="http://example.org/onto/class/google_cloud_run_service"/>
    <rdfs:range rdf:resource="http://www.w3.org/2001/XMLSchema#string"/>
  </owl:DatatypeProperty>
  <owl:DatatypeProperty rdf:about="http://example.org/onto/prop/google_cloud_run_service_default_mode">
    <rdfs:label>default_mode</rdfs:label>
    <rdfs:comment>Mode bits to use on created files by default. Must be a value between 0000
and 0777. Defaults to 0644. Directories within the path are not affected by
this setting. This might be in conflict with other options that affect the
file mode, like fsGroup, and the result can be other mode bits set.</rdfs:comment>
    <rdfs:domain rdf:resource="http://example.org/onto/class/google_cloud_run_service"/>
    <rdfs:range rdf:resource="http://www.w3.org/2001/XMLSchema#string"/>
  </owl:DatatypeProperty>
  <owl:DatatypeProperty rdf:about="http://example.org/onto/prop/google_cloud_run_service_secret_name">
    <rdfs:label>secret_name</rdfs:label>
    <rdfs:comment>The name of the secret in Cloud Secret Manager. By default, the secret
is assumed to be in the same project.
If the secret is in another project, you must define an alias.
An alias definition has the form:
{alias}:projects/{project-id|project-number}/secrets/{secret-name}.
If multiple alias definitions are needed, they must be separated by
commas.
The alias definitions must be set on the run.googleapis.com/secrets
annotation.</rdfs:comment>
    <rdfs:domain rdf:resource="http://example.org/onto/class/google_cloud_run_service"/>
    <rdfs:range rdf:resource="http://www.w3.org/2001/XMLSchema#string"/>
  </owl:DatatypeProperty>
  <owl:DatatypeProperty rdf:about="http://example.org/onto/prop/google_cloud_run_service_key">
    <rdfs:label>key</rdfs:label>
    <rdfs:comment>The Cloud Secret Manager secret version.
Can be 'latest' for the latest value or an integer for a specific version.</rdfs:comment>
    <rdfs:domain rdf:resource="http://example.org/onto/class/google_cloud_run_service"/>
    <rdfs:range rdf:resource="http://www.w3.org/2001/XMLSchema#string"/>
  </owl:DatatypeProperty>
  <owl:DatatypeProperty rdf:about="http://example.org/onto/prop/google_cloud_run_service_mode">
    <rdfs:label>mode</rdfs:label>
    <rdfs:comment>Mode bits to use on this file, must be a value between 0000 and 0777. If
not specified, the volume defaultMode will be used. This might be in
conflict with other options that affect the file mode, like fsGroup, and
the result can be other mode bits set.</rdfs:comment>
    <rdfs:domain rdf:resource="http://example.org/onto/class/google_cloud_run_service"/>
    <rdfs:range rdf:resource="http://www.w3.org/2001/XMLSchema#string"/>
  </owl:DatatypeProperty>
  <owl:DatatypeProperty rdf:about="http://example.org/onto/prop/google_cloud_run_service_path">
    <rdfs:label>path</rdfs:label>
    <rdfs:comment>The relative path of the file to map the key to.
May not be an absolute path.
May not contain the path element '..'.
May not start with the string '..'.</rdfs:comment>
    <rdfs:domain rdf:resource="http://example.org/onto/class/google_cloud_run_service"/>
    <rdfs:range rdf:resource="http://www.w3.org/2001/XMLSchema#string"/>
  </owl:DatatypeProperty>
  <owl:DatatypeProperty rdf:about="http://example.org/onto/prop/google_cloud_run_service_create">
    <rdfs:label>create</rdfs:label>
    <rdfs:domain rdf:resource="http://example.org/onto/class/google_cloud_run_service"/>
    <rdfs:range rdf:resource="http://www.w3.org/2001/XMLSchema#string"/>
  </owl:DatatypeProperty>
  <owl:DatatypeProperty rdf:about="http://example.org/onto/prop/google_cloud_run_service_delete">
    <rdfs:label>delete</rdfs:label>
    <rdfs:domain rdf:resource="http://example.org/onto/class/google_cloud_run_service"/>
    <rdfs:range rdf:resource="http://www.w3.org/2001/XMLSchema#string"/>
  </owl:DatatypeProperty>
  <owl:DatatypeProperty rdf:about="http://example.org/onto/prop/google_cloud_run_service_update">
    <rdfs:label>update</rdfs:label>
    <rdfs:domain rdf:resource="http://example.org/onto/class/google_cloud_run_service"/>
    <rdfs:range rdf:resource="http://www.w3.org/2001/XMLSchema#string"/>
  </owl:DatatypeProperty>
  <owl:DatatypeProperty rdf:about="http://example.org/onto/prop/google_cloud_run_service_latest_revision">
    <rdfs:label>latest_revision</rdfs:label>
    <rdfs:comment>LatestRevision may be optionally provided to indicate that the latest ready
Revision of the Configuration should be used for this traffic target. When
provided LatestRevision must be true if RevisionName is empty; it must be
false when RevisionName is non-empty.</rdfs:comment>
    <rdfs:domain rdf:resource="http://example.org/onto/class/google_cloud_run_service"/>
    <rdfs:range rdf:resource="http://www.w3.org/2001/XMLSchema#string"/>
  </owl:DatatypeProperty>
  <owl:DatatypeProperty rdf:about="http://example.org/onto/prop/google_cloud_run_service_percent">
    <rdfs:label>percent</rdfs:label>
    <rdfs:comment>Percent specifies percent of the traffic to this Revision or Configuration.</rdfs:comment>
    <rdfs:domain rdf:resource="http://example.org/onto/class/google_cloud_run_service"/>
    <rdfs:range rdf:resource="http://www.w3.org/2001/XMLSchema#string"/>
  </owl:DatatypeProperty>
  <owl:DatatypeProperty rdf:about="http://example.org/onto/prop/google_cloud_run_service_revision_name">
    <rdfs:label>revision_name</rdfs:label>
    <rdfs:comment>RevisionName of a specific revision to which to send this portion of traffic.</rdfs:comment>
    <rdfs:domain rdf:resource="http://example.org/onto/class/google_cloud_run_service"/>
    <rdfs:range rdf:resource="http://www.w3.org/2001/XMLSchema#string"/>
  </owl:DatatypeProperty>
  <owl:DatatypeProperty rdf:about="http://example.org/onto/prop/google_cloud_run_service_tag">
    <rdfs:label>tag</rdfs:label>
    <rdfs:comment>Tag is optionally used to expose a dedicated url for referencing this target exclusively.</rdfs:comment>
    <rdfs:domain rdf:resource="http://example.org/onto/class/google_cloud_run_service"/>
    <rdfs:range rdf:resource="http://www.w3.org/2001/XMLSchema#string"/>
  </owl:DatatypeProperty>
  <owl:DatatypeProperty rdf:about="http://example.org/onto/prop/google_cloud_run_service_url">
    <rdfs:label>url</rdfs:label>
    <rdfs:comment>URL displays the URL for accessing tagged traffic targets. URL is displayed in status,
and is disallowed on spec. URL must contain a scheme (e.g. http://) and a hostname,
but may not contain anything else (e.g. basic auth, url path, etc.)</rdfs:comment>
    <rdfs:domain rdf:resource="http://example.org/onto/class/google_cloud_run_service"/>
    <rdfs:range rdf:resource="http://www.w3.org/2001/XMLSchema#string"/>
  </owl:DatatypeProperty>
</rdf:RDF>
