<?xml version="1.0" encoding="UTF-8"?>
<rdf:RDF
  xmlns:rdf="http://www.w3.org/1999/02/22-rdf-syntax-ns#"
  xmlns:rdfs="http://www.w3.org/2000/01/rdf-schema#"
  xmlns:owl="http://www.w3.org/2002/07/owl#"
  xmlns:xsd="http://www.w3.org/2001/XMLSchema#"
  xml:base="http://example.org/onto/">
  <owl:Class rdf:about="http://example.org/onto/class/google_network_services_lb_traffic_extension">
    <rdfs:label>google_network_services_lb_traffic_extension</rdfs:label>
    <rdfs:comment>#
#     ***     AUTO GENERATED CODE    ***    Type: MMv1     ***
#
# ----------------------------------------------------------------------------
#
#     This code is generated by Magic Modules using the following:
#
#     Configuration: https:#github.com/GoogleCloudPlatform/magic-modules/tree/main/mmv1/products/networkservices/LbTrafficExtension.yaml
#     Template:      https:#github.com/GoogleCloudPlatform/magic-modules/tree/main/mmv1/templates/terraform/resource.html.markdown.tmpl
#
#     DO NOT EDIT this file directly. Any changes made to this file will be
#     overwritten during the next generation cycle.
#
# ----------------------------------------------------------------------------
subcategory: "Network Services"
description: |-
  LbTrafficExtension is a resource that lets the extension service modify the headers and payloads of both requests and responses without impacting the choice of backend services or any other security policies associated with the backend service.
---</rdfs:comment>
  </owl:Class>
  <owl:DatatypeProperty rdf:about="http://example.org/onto/prop/google_network_services_lb_traffic_extension_description">
    <rdfs:label>description</rdfs:label>
    <rdfs:comment>A human-readable description of the resource.</rdfs:comment>
    <rdfs:domain rdf:resource="http://example.org/onto/class/google_network_services_lb_traffic_extension"/>
    <rdfs:range rdf:resource="http://www.w3.org/2001/XMLSchema#string"/>
  </owl:DatatypeProperty>
  <owl:DatatypeProperty rdf:about="http://example.org/onto/prop/google_network_services_lb_traffic_extension_effective_labels">
    <rdfs:label>effective_labels</rdfs:label>
    <rdfs:comment>All of labels (key/value pairs) present on the resource in GCP, including the labels configured through Terraform, other clients and services.</rdfs:comment>
    <rdfs:domain rdf:resource="http://example.org/onto/class/google_network_services_lb_traffic_extension"/>
    <rdfs:range rdf:resource="http://www.w3.org/2001/XMLSchema#string"/>
  </owl:DatatypeProperty>
  <owl:DatatypeProperty rdf:about="http://example.org/onto/prop/google_network_services_lb_traffic_extension_forwarding_rules">
    <rdfs:label>forwarding_rules</rdfs:label>
    <rdfs:comment>A list of references to the forwarding rules to which this service extension is attached to.
At least one forwarding rule is required. There can be only one LBTrafficExtension resource per forwarding rule.</rdfs:comment>
    <rdfs:domain rdf:resource="http://example.org/onto/class/google_network_services_lb_traffic_extension"/>
    <rdfs:range rdf:resource="http://www.w3.org/2001/XMLSchema#string"/>
  </owl:DatatypeProperty>
  <owl:DatatypeProperty rdf:about="http://example.org/onto/prop/google_network_services_lb_traffic_extension_id">
    <rdfs:label>id</rdfs:label>
    <rdfs:domain rdf:resource="http://example.org/onto/class/google_network_services_lb_traffic_extension"/>
    <rdfs:range rdf:resource="http://www.w3.org/2001/XMLSchema#string"/>
  </owl:DatatypeProperty>
  <owl:DatatypeProperty rdf:about="http://example.org/onto/prop/google_network_services_lb_traffic_extension_labels">
    <rdfs:label>labels</rdfs:label>
    <rdfs:comment>Set of labels associated with the LbTrafficExtension resource.

**Note**: This field is non-authoritative, and will only manage the labels present in your configuration.
Please refer to the field 'effective_labels' for all of the labels present on the resource.</rdfs:comment>
    <rdfs:domain rdf:resource="http://example.org/onto/class/google_network_services_lb_traffic_extension"/>
    <rdfs:range rdf:resource="http://www.w3.org/2001/XMLSchema#string"/>
  </owl:DatatypeProperty>
  <owl:DatatypeProperty rdf:about="http://example.org/onto/prop/google_network_services_lb_traffic_extension_load_balancing_scheme">
    <rdfs:label>load_balancing_scheme</rdfs:label>
    <rdfs:comment>All backend services and forwarding rules referenced by this extension must share the same load balancing scheme.
For more information, refer to [Choosing a load balancer](https://cloud.google.com/load-balancing/docs/backend-service) and
[Supported application load balancers](https://cloud.google.com/service-extensions/docs/callouts-overview#supported-lbs). Possible values: ["INTERNAL_MANAGED", "EXTERNAL_MANAGED"]</rdfs:comment>
    <rdfs:domain rdf:resource="http://example.org/onto/class/google_network_services_lb_traffic_extension"/>
    <rdfs:range rdf:resource="http://www.w3.org/2001/XMLSchema#string"/>
  </owl:DatatypeProperty>
  <owl:DatatypeProperty rdf:about="http://example.org/onto/prop/google_network_services_lb_traffic_extension_location">
    <rdfs:label>location</rdfs:label>
    <rdfs:comment>The location of the traffic extension</rdfs:comment>
    <rdfs:domain rdf:resource="http://example.org/onto/class/google_network_services_lb_traffic_extension"/>
    <rdfs:range rdf:resource="http://www.w3.org/2001/XMLSchema#string"/>
  </owl:DatatypeProperty>
  <owl:DatatypeProperty rdf:about="http://example.org/onto/prop/google_network_services_lb_traffic_extension_name">
    <rdfs:label>name</rdfs:label>
    <rdfs:comment>Name of the LbTrafficExtension resource in the following format: projects/{project}/locations/{location}/lbTrafficExtensions/{lbTrafficExtension}.</rdfs:comment>
    <rdfs:domain rdf:resource="http://example.org/onto/class/google_network_services_lb_traffic_extension"/>
    <rdfs:range rdf:resource="http://www.w3.org/2001/XMLSchema#string"/>
  </owl:DatatypeProperty>
  <owl:DatatypeProperty rdf:about="http://example.org/onto/prop/google_network_services_lb_traffic_extension_project">
    <rdfs:label>project</rdfs:label>
    <rdfs:domain rdf:resource="http://example.org/onto/class/google_network_services_lb_traffic_extension"/>
    <rdfs:range rdf:resource="http://www.w3.org/2001/XMLSchema#string"/>
  </owl:DatatypeProperty>
  <owl:DatatypeProperty rdf:about="http://example.org/onto/prop/google_network_services_lb_traffic_extension_terraform_labels">
    <rdfs:label>terraform_labels</rdfs:label>
    <rdfs:comment>The combination of labels configured directly on the resource
 and default labels configured on the provider.</rdfs:comment>
    <rdfs:domain rdf:resource="http://example.org/onto/class/google_network_services_lb_traffic_extension"/>
    <rdfs:range rdf:resource="http://www.w3.org/2001/XMLSchema#string"/>
  </owl:DatatypeProperty>
  <owl:DatatypeProperty rdf:about="http://example.org/onto/prop/google_network_services_lb_traffic_extension_name">
    <rdfs:label>name</rdfs:label>
    <rdfs:comment>The name for this extension chain. The name is logged as part of the HTTP request logs.
The name must conform with RFC-1034, is restricted to lower-cased letters, numbers and hyphens,
and can have a maximum length of 63 characters. Additionally, the first character must be a letter
and the last a letter or a number.</rdfs:comment>
    <rdfs:domain rdf:resource="http://example.org/onto/class/google_network_services_lb_traffic_extension"/>
    <rdfs:range rdf:resource="http://www.w3.org/2001/XMLSchema#string"/>
  </owl:DatatypeProperty>
  <owl:DatatypeProperty rdf:about="http://example.org/onto/prop/google_network_services_lb_traffic_extension_authority">
    <rdfs:label>authority</rdfs:label>
    <rdfs:comment>The :authority header in the gRPC request sent from Envoy to the extension service.</rdfs:comment>
    <rdfs:domain rdf:resource="http://example.org/onto/class/google_network_services_lb_traffic_extension"/>
    <rdfs:range rdf:resource="http://www.w3.org/2001/XMLSchema#string"/>
  </owl:DatatypeProperty>
  <owl:DatatypeProperty rdf:about="http://example.org/onto/prop/google_network_services_lb_traffic_extension_fail_open">
    <rdfs:label>fail_open</rdfs:label>
    <rdfs:comment>Determines how the proxy behaves if the call to the extension fails or times out.
When set to TRUE, request or response processing continues without error.
Any subsequent extensions in the extension chain are also executed.
When set to FALSE: * If response headers have not been delivered to the downstream client,
a generic 500 error is returned to the client. The error response can be tailored by
configuring a custom error response in the load balancer.</rdfs:comment>
    <rdfs:domain rdf:resource="http://example.org/onto/class/google_network_services_lb_traffic_extension"/>
    <rdfs:range rdf:resource="http://www.w3.org/2001/XMLSchema#string"/>
  </owl:DatatypeProperty>
  <owl:DatatypeProperty rdf:about="http://example.org/onto/prop/google_network_services_lb_traffic_extension_forward_headers">
    <rdfs:label>forward_headers</rdfs:label>
    <rdfs:comment>List of the HTTP headers to forward to the extension (from the client or backend).
If omitted, all headers are sent. Each element is a string indicating the header name.</rdfs:comment>
    <rdfs:domain rdf:resource="http://example.org/onto/class/google_network_services_lb_traffic_extension"/>
    <rdfs:range rdf:resource="http://www.w3.org/2001/XMLSchema#string"/>
  </owl:DatatypeProperty>
  <owl:DatatypeProperty rdf:about="http://example.org/onto/prop/google_network_services_lb_traffic_extension_metadata">
    <rdfs:label>metadata</rdfs:label>
    <rdfs:comment>Metadata associated with the extension. This field is used to pass metadata to the extension service.
You can set up key value pairs for metadata as you like and need.
f.e. {"key": "value", "key2": "value2"}.</rdfs:comment>
    <rdfs:domain rdf:resource="http://example.org/onto/class/google_network_services_lb_traffic_extension"/>
    <rdfs:range rdf:resource="http://www.w3.org/2001/XMLSchema#string"/>
  </owl:DatatypeProperty>
  <owl:DatatypeProperty rdf:about="http://example.org/onto/prop/google_network_services_lb_traffic_extension_name">
    <rdfs:label>name</rdfs:label>
    <rdfs:comment>The name for this extension. The name is logged as part of the HTTP request logs.
The name must conform with RFC-1034, is restricted to lower-cased letters, numbers and hyphens,
and can have a maximum length of 63 characters. Additionally, the first character must be a letter
and the last a letter or a number.</rdfs:comment>
    <rdfs:domain rdf:resource="http://example.org/onto/class/google_network_services_lb_traffic_extension"/>
    <rdfs:range rdf:resource="http://www.w3.org/2001/XMLSchema#string"/>
  </owl:DatatypeProperty>
  <owl:DatatypeProperty rdf:about="http://example.org/onto/prop/google_network_services_lb_traffic_extension_service">
    <rdfs:label>service</rdfs:label>
    <rdfs:comment>The reference to the service that runs the extension.

* To configure a callout extension, service must be a fully-qualified reference to a backend service.
* To configure a plugin extension, service must be a reference to a WasmPlugin resource.</rdfs:comment>
    <rdfs:domain rdf:resource="http://example.org/onto/class/google_network_services_lb_traffic_extension"/>
    <rdfs:range rdf:resource="http://www.w3.org/2001/XMLSchema#string"/>
  </owl:DatatypeProperty>
  <owl:DatatypeProperty rdf:about="http://example.org/onto/prop/google_network_services_lb_traffic_extension_supported_events">
    <rdfs:label>supported_events</rdfs:label>
    <rdfs:comment>A set of events during request or response processing for which this extension is called.
This field is required for the LbTrafficExtension resource. It's not relevant for the LbRouteExtension
resource. Possible values:'EVENT_TYPE_UNSPECIFIED', 'REQUEST_HEADERS', 'REQUEST_BODY', 'RESPONSE_HEADERS',
'RESPONSE_BODY', 'RESPONSE_BODY' and 'RESPONSE_BODY'.</rdfs:comment>
    <rdfs:domain rdf:resource="http://example.org/onto/class/google_network_services_lb_traffic_extension"/>
    <rdfs:range rdf:resource="http://www.w3.org/2001/XMLSchema#string"/>
  </owl:DatatypeProperty>
  <owl:DatatypeProperty rdf:about="http://example.org/onto/prop/google_network_services_lb_traffic_extension_timeout">
    <rdfs:label>timeout</rdfs:label>
    <rdfs:comment>Specifies the timeout for each individual message on the stream. The timeout must be between 10-1000 milliseconds.
A duration in seconds with up to nine fractional digits, ending with 's'. Example: "3.5s".</rdfs:comment>
    <rdfs:domain rdf:resource="http://example.org/onto/class/google_network_services_lb_traffic_extension"/>
    <rdfs:range rdf:resource="http://www.w3.org/2001/XMLSchema#string"/>
  </owl:DatatypeProperty>
  <owl:DatatypeProperty rdf:about="http://example.org/onto/prop/google_network_services_lb_traffic_extension_cel_expression">
    <rdfs:label>cel_expression</rdfs:label>
    <rdfs:comment>A Common Expression Language (CEL) expression that is used to match requests for which the extension chain is executed.</rdfs:comment>
    <rdfs:domain rdf:resource="http://example.org/onto/class/google_network_services_lb_traffic_extension"/>
    <rdfs:range rdf:resource="http://www.w3.org/2001/XMLSchema#string"/>
  </owl:DatatypeProperty>
  <owl:DatatypeProperty rdf:about="http://example.org/onto/prop/google_network_services_lb_traffic_extension_create">
    <rdfs:label>create</rdfs:label>
    <rdfs:domain rdf:resource="http://example.org/onto/class/google_network_services_lb_traffic_extension"/>
    <rdfs:range rdf:resource="http://www.w3.org/2001/XMLSchema#string"/>
  </owl:DatatypeProperty>
  <owl:DatatypeProperty rdf:about="http://example.org/onto/prop/google_network_services_lb_traffic_extension_delete">
    <rdfs:label>delete</rdfs:label>
    <rdfs:domain rdf:resource="http://example.org/onto/class/google_network_services_lb_traffic_extension"/>
    <rdfs:range rdf:resource="http://www.w3.org/2001/XMLSchema#string"/>
  </owl:DatatypeProperty>
  <owl:DatatypeProperty rdf:about="http://example.org/onto/prop/google_network_services_lb_traffic_extension_update">
    <rdfs:label>update</rdfs:label>
    <rdfs:domain rdf:resource="http://example.org/onto/class/google_network_services_lb_traffic_extension"/>
    <rdfs:range rdf:resource="http://www.w3.org/2001/XMLSchema#string"/>
  </owl:DatatypeProperty>
</rdf:RDF>
