<?xml version="1.0" encoding="UTF-8"?>
<rdf:RDF
  xmlns:rdf="http://www.w3.org/1999/02/22-rdf-syntax-ns#"
  xmlns:rdfs="http://www.w3.org/2000/01/rdf-schema#"
  xmlns:owl="http://www.w3.org/2002/07/owl#"
  xmlns:xsd="http://www.w3.org/2001/XMLSchema#"
  xml:base="http://example.org/onto/">
  <owl:Class rdf:about="http://example.org/onto/class/google_cloud_run_v2_worker_pool">
    <rdfs:label>google_cloud_run_v2_worker_pool</rdfs:label>
    <rdfs:comment>#
#     ***     AUTO GENERATED CODE    ***    Type: MMv1     ***
#
# ----------------------------------------------------------------------------
#
#     This code is generated by Magic Modules using the following:
#
#     Configuration: https:#github.com/GoogleCloudPlatform/magic-modules/tree/main/mmv1/products/cloudrunv2/WorkerPool.yaml
#     Template:      https:#github.com/GoogleCloudPlatform/magic-modules/tree/main/mmv1/templates/terraform/resource.html.markdown.tmpl
#
#     DO NOT EDIT this file directly. Any changes made to this file will be
#     overwritten during the next generation cycle.
#
# ----------------------------------------------------------------------------
subcategory: "Cloud Run (v2 API)"
description: |-
  WorkerPool acts as a top-level container that manages a set of configurations and revision templates which implement a pull-based workload.
---</rdfs:comment>
  </owl:Class>
  <owl:DatatypeProperty rdf:about="http://example.org/onto/prop/google_cloud_run_v2_worker_pool_annotations">
    <rdfs:label>annotations</rdfs:label>
    <rdfs:comment>Unstructured key value map that may be set by external tools to store and arbitrary metadata. They are not queryable and should be preserved when modifying objects.

Cloud Run API v2 does not support annotations with 'run.googleapis.com', 'cloud.googleapis.com', 'serving.knative.dev', or 'autoscaling.knative.dev' namespaces, and they will be rejected in new resources.
All system annotations in v1 now have a corresponding field in v2 WorkerPool.

This field follows Kubernetes annotations' namespacing, limits, and rules.

**Note**: This field is non-authoritative, and will only manage the annotations present in your configuration.
Please refer to the field 'effective_annotations' for all of the annotations present on the resource.</rdfs:comment>
    <rdfs:domain rdf:resource="http://example.org/onto/class/google_cloud_run_v2_worker_pool"/>
    <rdfs:range rdf:resource="http://www.w3.org/2001/XMLSchema#string"/>
  </owl:DatatypeProperty>
  <owl:DatatypeProperty rdf:about="http://example.org/onto/prop/google_cloud_run_v2_worker_pool_client">
    <rdfs:label>client</rdfs:label>
    <rdfs:comment>Arbitrary identifier for the API client.</rdfs:comment>
    <rdfs:domain rdf:resource="http://example.org/onto/class/google_cloud_run_v2_worker_pool"/>
    <rdfs:range rdf:resource="http://www.w3.org/2001/XMLSchema#string"/>
  </owl:DatatypeProperty>
  <owl:DatatypeProperty rdf:about="http://example.org/onto/prop/google_cloud_run_v2_worker_pool_client_version">
    <rdfs:label>client_version</rdfs:label>
    <rdfs:comment>Arbitrary version identifier for the API client.</rdfs:comment>
    <rdfs:domain rdf:resource="http://example.org/onto/class/google_cloud_run_v2_worker_pool"/>
    <rdfs:range rdf:resource="http://www.w3.org/2001/XMLSchema#string"/>
  </owl:DatatypeProperty>
  <owl:DatatypeProperty rdf:about="http://example.org/onto/prop/google_cloud_run_v2_worker_pool_conditions">
    <rdfs:label>conditions</rdfs:label>
    <rdfs:comment>The Conditions of all other associated sub-resources. They contain additional diagnostics information in case the WorkerPool does not reach its Serving state. See comments in reconciling for additional information on reconciliation process in Cloud Run.</rdfs:comment>
    <rdfs:domain rdf:resource="http://example.org/onto/class/google_cloud_run_v2_worker_pool"/>
    <rdfs:range rdf:resource="http://www.w3.org/2001/XMLSchema#string"/>
  </owl:DatatypeProperty>
  <owl:DatatypeProperty rdf:about="http://example.org/onto/prop/google_cloud_run_v2_worker_pool_create_time">
    <rdfs:label>create_time</rdfs:label>
    <rdfs:comment>The creation time.</rdfs:comment>
    <rdfs:domain rdf:resource="http://example.org/onto/class/google_cloud_run_v2_worker_pool"/>
    <rdfs:range rdf:resource="http://www.w3.org/2001/XMLSchema#string"/>
  </owl:DatatypeProperty>
  <owl:DatatypeProperty rdf:about="http://example.org/onto/prop/google_cloud_run_v2_worker_pool_creator">
    <rdfs:label>creator</rdfs:label>
    <rdfs:comment>Email address of the authenticated creator.</rdfs:comment>
    <rdfs:domain rdf:resource="http://example.org/onto/class/google_cloud_run_v2_worker_pool"/>
    <rdfs:range rdf:resource="http://www.w3.org/2001/XMLSchema#string"/>
  </owl:DatatypeProperty>
  <owl:DatatypeProperty rdf:about="http://example.org/onto/prop/google_cloud_run_v2_worker_pool_custom_audiences">
    <rdfs:label>custom_audiences</rdfs:label>
    <rdfs:comment>One or more custom audiences that you want this worker pool to support. Specify each custom audience as the full URL in a string. The custom audiences are encoded in the token and used to authenticate requests.
For more information, see https://cloud.google.com/run/docs/configuring/custom-audiences.</rdfs:comment>
    <rdfs:domain rdf:resource="http://example.org/onto/class/google_cloud_run_v2_worker_pool"/>
    <rdfs:range rdf:resource="http://www.w3.org/2001/XMLSchema#string"/>
  </owl:DatatypeProperty>
  <owl:DatatypeProperty rdf:about="http://example.org/onto/prop/google_cloud_run_v2_worker_pool_delete_time">
    <rdfs:label>delete_time</rdfs:label>
    <rdfs:comment>The deletion time.</rdfs:comment>
    <rdfs:domain rdf:resource="http://example.org/onto/class/google_cloud_run_v2_worker_pool"/>
    <rdfs:range rdf:resource="http://www.w3.org/2001/XMLSchema#string"/>
  </owl:DatatypeProperty>
  <owl:DatatypeProperty rdf:about="http://example.org/onto/prop/google_cloud_run_v2_worker_pool_deletion_protection">
    <rdfs:label>deletion_protection</rdfs:label>
    <rdfs:comment>Whether Terraform will be prevented from destroying the service. Defaults to true.
When a'terraform destroy' or 'terraform apply' would delete the service,
the command will fail if this field is not set to false in Terraform state.
When the field is set to true or unset in Terraform state, a 'terraform apply'
or 'terraform destroy' that would delete the WorkerPool will fail.
When the field is set to false, deleting the WorkerPool is allowed.</rdfs:comment>
    <rdfs:domain rdf:resource="http://example.org/onto/class/google_cloud_run_v2_worker_pool"/>
    <rdfs:range rdf:resource="http://www.w3.org/2001/XMLSchema#string"/>
  </owl:DatatypeProperty>
  <owl:DatatypeProperty rdf:about="http://example.org/onto/prop/google_cloud_run_v2_worker_pool_description">
    <rdfs:label>description</rdfs:label>
    <rdfs:comment>User-provided description of the WorkerPool. This field currently has a 512-character limit.</rdfs:comment>
    <rdfs:domain rdf:resource="http://example.org/onto/class/google_cloud_run_v2_worker_pool"/>
    <rdfs:range rdf:resource="http://www.w3.org/2001/XMLSchema#string"/>
  </owl:DatatypeProperty>
  <owl:DatatypeProperty rdf:about="http://example.org/onto/prop/google_cloud_run_v2_worker_pool_effective_annotations">
    <rdfs:label>effective_annotations</rdfs:label>
    <rdfs:comment>All of annotations (key/value pairs) present on the resource in GCP, including the annotations configured through Terraform, other clients and services.</rdfs:comment>
    <rdfs:domain rdf:resource="http://example.org/onto/class/google_cloud_run_v2_worker_pool"/>
    <rdfs:range rdf:resource="http://www.w3.org/2001/XMLSchema#string"/>
  </owl:DatatypeProperty>
  <owl:DatatypeProperty rdf:about="http://example.org/onto/prop/google_cloud_run_v2_worker_pool_effective_labels">
    <rdfs:label>effective_labels</rdfs:label>
    <rdfs:comment>All of labels (key/value pairs) present on the resource in GCP, including the labels configured through Terraform, other clients and services.</rdfs:comment>
    <rdfs:domain rdf:resource="http://example.org/onto/class/google_cloud_run_v2_worker_pool"/>
    <rdfs:range rdf:resource="http://www.w3.org/2001/XMLSchema#string"/>
  </owl:DatatypeProperty>
  <owl:DatatypeProperty rdf:about="http://example.org/onto/prop/google_cloud_run_v2_worker_pool_etag">
    <rdfs:label>etag</rdfs:label>
    <rdfs:comment>A system-generated fingerprint for this version of the resource. May be used to detect modification conflict during updates.</rdfs:comment>
    <rdfs:domain rdf:resource="http://example.org/onto/class/google_cloud_run_v2_worker_pool"/>
    <rdfs:range rdf:resource="http://www.w3.org/2001/XMLSchema#string"/>
  </owl:DatatypeProperty>
  <owl:DatatypeProperty rdf:about="http://example.org/onto/prop/google_cloud_run_v2_worker_pool_expire_time">
    <rdfs:label>expire_time</rdfs:label>
    <rdfs:comment>For a deleted resource, the time after which it will be permanently deleted.</rdfs:comment>
    <rdfs:domain rdf:resource="http://example.org/onto/class/google_cloud_run_v2_worker_pool"/>
    <rdfs:range rdf:resource="http://www.w3.org/2001/XMLSchema#string"/>
  </owl:DatatypeProperty>
  <owl:DatatypeProperty rdf:about="http://example.org/onto/prop/google_cloud_run_v2_worker_pool_generation">
    <rdfs:label>generation</rdfs:label>
    <rdfs:comment>A number that monotonically increases every time the user modifies the desired state. Please note that unlike v1, this is an int64 value. As with most Google APIs, its JSON representation will be a string instead of an integer.</rdfs:comment>
    <rdfs:domain rdf:resource="http://example.org/onto/class/google_cloud_run_v2_worker_pool"/>
    <rdfs:range rdf:resource="http://www.w3.org/2001/XMLSchema#string"/>
  </owl:DatatypeProperty>
  <owl:DatatypeProperty rdf:about="http://example.org/onto/prop/google_cloud_run_v2_worker_pool_id">
    <rdfs:label>id</rdfs:label>
    <rdfs:domain rdf:resource="http://example.org/onto/class/google_cloud_run_v2_worker_pool"/>
    <rdfs:range rdf:resource="http://www.w3.org/2001/XMLSchema#string"/>
  </owl:DatatypeProperty>
  <owl:DatatypeProperty rdf:about="http://example.org/onto/prop/google_cloud_run_v2_worker_pool_instance_split_statuses">
    <rdfs:label>instance_split_statuses</rdfs:label>
    <rdfs:comment>Detailed status information for corresponding instance splits. See comments in reconciling for additional information on reconciliation process in Cloud Run.</rdfs:comment>
    <rdfs:domain rdf:resource="http://example.org/onto/class/google_cloud_run_v2_worker_pool"/>
    <rdfs:range rdf:resource="http://www.w3.org/2001/XMLSchema#string"/>
  </owl:DatatypeProperty>
  <owl:DatatypeProperty rdf:about="http://example.org/onto/prop/google_cloud_run_v2_worker_pool_labels">
    <rdfs:label>labels</rdfs:label>
    <rdfs:comment>Unstructured key value map that can be used to organize and categorize objects. User-provided labels are shared with Google's billing system, so they can be used to filter, or break down billing charges by team, component,
environment, state, etc. For more information, visit https://cloud.google.com/resource-manager/docs/creating-managing-labels or https://cloud.google.com/run/docs/configuring/labels.

Cloud Run API v2 does not support labels with  'run.googleapis.com', 'cloud.googleapis.com', 'serving.knative.dev', or 'autoscaling.knative.dev' namespaces, and they will be rejected.
All system labels in v1 now have a corresponding field in v2 WorkerPool.

**Note**: This field is non-authoritative, and will only manage the labels present in your configuration.
Please refer to the field 'effective_labels' for all of the labels present on the resource.</rdfs:comment>
    <rdfs:domain rdf:resource="http://example.org/onto/class/google_cloud_run_v2_worker_pool"/>
    <rdfs:range rdf:resource="http://www.w3.org/2001/XMLSchema#string"/>
  </owl:DatatypeProperty>
  <owl:DatatypeProperty rdf:about="http://example.org/onto/prop/google_cloud_run_v2_worker_pool_last_modifier">
    <rdfs:label>last_modifier</rdfs:label>
    <rdfs:comment>Email address of the last authenticated modifier.</rdfs:comment>
    <rdfs:domain rdf:resource="http://example.org/onto/class/google_cloud_run_v2_worker_pool"/>
    <rdfs:range rdf:resource="http://www.w3.org/2001/XMLSchema#string"/>
  </owl:DatatypeProperty>
  <owl:DatatypeProperty rdf:about="http://example.org/onto/prop/google_cloud_run_v2_worker_pool_latest_created_revision">
    <rdfs:label>latest_created_revision</rdfs:label>
    <rdfs:comment>Name of the last created revision. See comments in reconciling for additional information on reconciliation process in Cloud Run.</rdfs:comment>
    <rdfs:domain rdf:resource="http://example.org/onto/class/google_cloud_run_v2_worker_pool"/>
    <rdfs:range rdf:resource="http://www.w3.org/2001/XMLSchema#string"/>
  </owl:DatatypeProperty>
  <owl:DatatypeProperty rdf:about="http://example.org/onto/prop/google_cloud_run_v2_worker_pool_latest_ready_revision">
    <rdfs:label>latest_ready_revision</rdfs:label>
    <rdfs:comment>Name of the latest revision that is serving traffic. See comments in reconciling for additional information on reconciliation process in Cloud Run.</rdfs:comment>
    <rdfs:domain rdf:resource="http://example.org/onto/class/google_cloud_run_v2_worker_pool"/>
    <rdfs:range rdf:resource="http://www.w3.org/2001/XMLSchema#string"/>
  </owl:DatatypeProperty>
  <owl:DatatypeProperty rdf:about="http://example.org/onto/prop/google_cloud_run_v2_worker_pool_launch_stage">
    <rdfs:label>launch_stage</rdfs:label>
    <rdfs:comment>The launch stage as defined by [Google Cloud Platform Launch Stages](https://cloud.google.com/products#product-launch-stages). Cloud Run supports ALPHA, BETA, and GA.
If no value is specified, GA is assumed. Set the launch stage to a preview stage on input to allow use of preview features in that stage. On read (or output), describes whether the resource uses preview features.

For example, if ALPHA is provided as input, but only BETA and GA-level features are used, this field will be BETA on output. Possible values: ["UNIMPLEMENTED", "PRELAUNCH", "EARLY_ACCESS", "ALPHA", "BETA", "GA", "DEPRECATED"]</rdfs:comment>
    <rdfs:domain rdf:resource="http://example.org/onto/class/google_cloud_run_v2_worker_pool"/>
    <rdfs:range rdf:resource="http://www.w3.org/2001/XMLSchema#string"/>
  </owl:DatatypeProperty>
  <owl:DatatypeProperty rdf:about="http://example.org/onto/prop/google_cloud_run_v2_worker_pool_location">
    <rdfs:label>location</rdfs:label>
    <rdfs:comment>The location of the cloud run worker pool</rdfs:comment>
    <rdfs:domain rdf:resource="http://example.org/onto/class/google_cloud_run_v2_worker_pool"/>
    <rdfs:range rdf:resource="http://www.w3.org/2001/XMLSchema#string"/>
  </owl:DatatypeProperty>
  <owl:DatatypeProperty rdf:about="http://example.org/onto/prop/google_cloud_run_v2_worker_pool_name">
    <rdfs:label>name</rdfs:label>
    <rdfs:comment>Name of the WorkerPool.</rdfs:comment>
    <rdfs:domain rdf:resource="http://example.org/onto/class/google_cloud_run_v2_worker_pool"/>
    <rdfs:range rdf:resource="http://www.w3.org/2001/XMLSchema#string"/>
  </owl:DatatypeProperty>
  <owl:DatatypeProperty rdf:about="http://example.org/onto/prop/google_cloud_run_v2_worker_pool_observed_generation">
    <rdfs:label>observed_generation</rdfs:label>
    <rdfs:comment>The generation of this WorkerPool currently serving traffic. See comments in reconciling for additional information on reconciliation process in Cloud Run. Please note that unlike v1, this is an int64 value. As with most Google APIs, its JSON representation will be a string instead of an integer.</rdfs:comment>
    <rdfs:domain rdf:resource="http://example.org/onto/class/google_cloud_run_v2_worker_pool"/>
    <rdfs:range rdf:resource="http://www.w3.org/2001/XMLSchema#string"/>
  </owl:DatatypeProperty>
  <owl:DatatypeProperty rdf:about="http://example.org/onto/prop/google_cloud_run_v2_worker_pool_project">
    <rdfs:label>project</rdfs:label>
    <rdfs:domain rdf:resource="http://example.org/onto/class/google_cloud_run_v2_worker_pool"/>
    <rdfs:range rdf:resource="http://www.w3.org/2001/XMLSchema#string"/>
  </owl:DatatypeProperty>
  <owl:DatatypeProperty rdf:about="http://example.org/onto/prop/google_cloud_run_v2_worker_pool_reconciling">
    <rdfs:label>reconciling</rdfs:label>
    <rdfs:comment>Returns true if the WorkerPool is currently being acted upon by the system to bring it into the desired state.

When a new WorkerPool is created, or an existing one is updated, Cloud Run will asynchronously perform all necessary steps to bring the WorkerPool to the desired serving state. This process is called reconciliation. While reconciliation is in process, observedGeneration, latest_ready_revison, trafficStatuses, and uri will have transient values that might mismatch the intended state: Once reconciliation is over (and this field is false), there are two possible outcomes: reconciliation succeeded and the serving state matches the WorkerPool, or there was an error, and reconciliation failed. This state can be found in terminalCondition.state.

If reconciliation succeeded, the following fields will match: traffic and trafficStatuses, observedGeneration and generation, latestReadyRevision and latestCreatedRevision.

If reconciliation failed, trafficStatuses, observedGeneration, and latestReadyRevision will have the state of the last serving revision, or empty for newly created WorkerPools. Additional information on the failure can be found in terminalCondition and conditions.</rdfs:comment>
    <rdfs:domain rdf:resource="http://example.org/onto/class/google_cloud_run_v2_worker_pool"/>
    <rdfs:range rdf:resource="http://www.w3.org/2001/XMLSchema#string"/>
  </owl:DatatypeProperty>
  <owl:DatatypeProperty rdf:about="http://example.org/onto/prop/google_cloud_run_v2_worker_pool_terminal_condition">
    <rdfs:label>terminal_condition</rdfs:label>
    <rdfs:comment>The Condition of this WorkerPool, containing its readiness status, and detailed error information in case it did not reach a serving state. See comments in reconciling for additional information on reconciliation process in Cloud Run.</rdfs:comment>
    <rdfs:domain rdf:resource="http://example.org/onto/class/google_cloud_run_v2_worker_pool"/>
    <rdfs:range rdf:resource="http://www.w3.org/2001/XMLSchema#string"/>
  </owl:DatatypeProperty>
  <owl:DatatypeProperty rdf:about="http://example.org/onto/prop/google_cloud_run_v2_worker_pool_terraform_labels">
    <rdfs:label>terraform_labels</rdfs:label>
    <rdfs:comment>The combination of labels configured directly on the resource
 and default labels configured on the provider.</rdfs:comment>
    <rdfs:domain rdf:resource="http://example.org/onto/class/google_cloud_run_v2_worker_pool"/>
    <rdfs:range rdf:resource="http://www.w3.org/2001/XMLSchema#string"/>
  </owl:DatatypeProperty>
  <owl:DatatypeProperty rdf:about="http://example.org/onto/prop/google_cloud_run_v2_worker_pool_uid">
    <rdfs:label>uid</rdfs:label>
    <rdfs:comment>Server assigned unique identifier for the trigger. The value is a UUID4 string and guaranteed to remain unchanged until the resource is deleted.</rdfs:comment>
    <rdfs:domain rdf:resource="http://example.org/onto/class/google_cloud_run_v2_worker_pool"/>
    <rdfs:range rdf:resource="http://www.w3.org/2001/XMLSchema#string"/>
  </owl:DatatypeProperty>
  <owl:DatatypeProperty rdf:about="http://example.org/onto/prop/google_cloud_run_v2_worker_pool_update_time">
    <rdfs:label>update_time</rdfs:label>
    <rdfs:comment>The last-modified time.</rdfs:comment>
    <rdfs:domain rdf:resource="http://example.org/onto/class/google_cloud_run_v2_worker_pool"/>
    <rdfs:range rdf:resource="http://www.w3.org/2001/XMLSchema#string"/>
  </owl:DatatypeProperty>
  <owl:DatatypeProperty rdf:about="http://example.org/onto/prop/google_cloud_run_v2_worker_pool_breakglass_justification">
    <rdfs:label>breakglass_justification</rdfs:label>
    <rdfs:comment>If present, indicates to use Breakglass using this justification. If useDefault is False, then it must be empty. For more information on breakglass, see https://cloud.google.com/binary-authorization/docs/using-breakglass</rdfs:comment>
    <rdfs:domain rdf:resource="http://example.org/onto/class/google_cloud_run_v2_worker_pool"/>
    <rdfs:range rdf:resource="http://www.w3.org/2001/XMLSchema#string"/>
  </owl:DatatypeProperty>
  <owl:DatatypeProperty rdf:about="http://example.org/onto/prop/google_cloud_run_v2_worker_pool_policy">
    <rdfs:label>policy</rdfs:label>
    <rdfs:comment>The path to a binary authorization policy. Format: projects/{project}/platforms/cloudRun/{policy-name}</rdfs:comment>
    <rdfs:domain rdf:resource="http://example.org/onto/class/google_cloud_run_v2_worker_pool"/>
    <rdfs:range rdf:resource="http://www.w3.org/2001/XMLSchema#string"/>
  </owl:DatatypeProperty>
  <owl:DatatypeProperty rdf:about="http://example.org/onto/prop/google_cloud_run_v2_worker_pool_use_default">
    <rdfs:label>use_default</rdfs:label>
    <rdfs:comment>If True, indicates to use the default project's binary authorization policy. If False, binary authorization will be disabled.</rdfs:comment>
    <rdfs:domain rdf:resource="http://example.org/onto/class/google_cloud_run_v2_worker_pool"/>
    <rdfs:range rdf:resource="http://www.w3.org/2001/XMLSchema#string"/>
  </owl:DatatypeProperty>
  <owl:DatatypeProperty rdf:about="http://example.org/onto/prop/google_cloud_run_v2_worker_pool_percent">
    <rdfs:label>percent</rdfs:label>
    <rdfs:comment>Specifies percent of the instance split to this Revision. This defaults to zero if unspecified.</rdfs:comment>
    <rdfs:domain rdf:resource="http://example.org/onto/class/google_cloud_run_v2_worker_pool"/>
    <rdfs:range rdf:resource="http://www.w3.org/2001/XMLSchema#string"/>
  </owl:DatatypeProperty>
  <owl:DatatypeProperty rdf:about="http://example.org/onto/prop/google_cloud_run_v2_worker_pool_revision">
    <rdfs:label>revision</rdfs:label>
    <rdfs:comment>Revision to which to assign this portion of instances, if split allocation is by revision.</rdfs:comment>
    <rdfs:domain rdf:resource="http://example.org/onto/class/google_cloud_run_v2_worker_pool"/>
    <rdfs:range rdf:resource="http://www.w3.org/2001/XMLSchema#string"/>
  </owl:DatatypeProperty>
  <owl:DatatypeProperty rdf:about="http://example.org/onto/prop/google_cloud_run_v2_worker_pool_type">
    <rdfs:label>type</rdfs:label>
    <rdfs:comment>The allocation type for this instance split. Possible values: ["INSTANCE_SPLIT_ALLOCATION_TYPE_LATEST", "INSTANCE_SPLIT_ALLOCATION_TYPE_REVISION"]</rdfs:comment>
    <rdfs:domain rdf:resource="http://example.org/onto/class/google_cloud_run_v2_worker_pool"/>
    <rdfs:range rdf:resource="http://www.w3.org/2001/XMLSchema#string"/>
  </owl:DatatypeProperty>
  <owl:DatatypeProperty rdf:about="http://example.org/onto/prop/google_cloud_run_v2_worker_pool_manual_instance_count">
    <rdfs:label>manual_instance_count</rdfs:label>
    <rdfs:comment>The total number of instances in manual scaling mode.</rdfs:comment>
    <rdfs:domain rdf:resource="http://example.org/onto/class/google_cloud_run_v2_worker_pool"/>
    <rdfs:range rdf:resource="http://www.w3.org/2001/XMLSchema#string"/>
  </owl:DatatypeProperty>
  <owl:DatatypeProperty rdf:about="http://example.org/onto/prop/google_cloud_run_v2_worker_pool_max_instance_count">
    <rdfs:label>max_instance_count</rdfs:label>
    <rdfs:comment>The maximum count of instances distributed among revisions based on the specified instance split percentages.</rdfs:comment>
    <rdfs:domain rdf:resource="http://example.org/onto/class/google_cloud_run_v2_worker_pool"/>
    <rdfs:range rdf:resource="http://www.w3.org/2001/XMLSchema#string"/>
  </owl:DatatypeProperty>
  <owl:DatatypeProperty rdf:about="http://example.org/onto/prop/google_cloud_run_v2_worker_pool_min_instance_count">
    <rdfs:label>min_instance_count</rdfs:label>
    <rdfs:comment>The minimum count of instances distributed among revisions based on the specified instance split percentages.</rdfs:comment>
    <rdfs:domain rdf:resource="http://example.org/onto/class/google_cloud_run_v2_worker_pool"/>
    <rdfs:range rdf:resource="http://www.w3.org/2001/XMLSchema#string"/>
  </owl:DatatypeProperty>
  <owl:DatatypeProperty rdf:about="http://example.org/onto/prop/google_cloud_run_v2_worker_pool_scaling_mode">
    <rdfs:label>scaling_mode</rdfs:label>
    <rdfs:comment>The scaling mode for the worker pool. It defaults to MANUAL. Possible values: ["AUTOMATIC", "MANUAL"]</rdfs:comment>
    <rdfs:domain rdf:resource="http://example.org/onto/class/google_cloud_run_v2_worker_pool"/>
    <rdfs:range rdf:resource="http://www.w3.org/2001/XMLSchema#string"/>
  </owl:DatatypeProperty>
  <owl:DatatypeProperty rdf:about="http://example.org/onto/prop/google_cloud_run_v2_worker_pool_annotations">
    <rdfs:label>annotations</rdfs:label>
    <rdfs:comment>Unstructured key value map that may be set by external tools to store and arbitrary metadata. They are not queryable and should be preserved when modifying objects.

Cloud Run API v2 does not support annotations with 'run.googleapis.com', 'cloud.googleapis.com', 'serving.knative.dev', or 'autoscaling.knative.dev' namespaces, and they will be rejected.
All system annotations in v1 now have a corresponding field in v2 WorkerPoolRevisionTemplate.

This field follows Kubernetes annotations' namespacing, limits, and rules.</rdfs:comment>
    <rdfs:domain rdf:resource="http://example.org/onto/class/google_cloud_run_v2_worker_pool"/>
    <rdfs:range rdf:resource="http://www.w3.org/2001/XMLSchema#string"/>
  </owl:DatatypeProperty>
  <owl:DatatypeProperty rdf:about="http://example.org/onto/prop/google_cloud_run_v2_worker_pool_encryption_key">
    <rdfs:label>encryption_key</rdfs:label>
    <rdfs:comment>A reference to a customer managed encryption key (CMEK) to use to encrypt this container image. For more information, go to https://cloud.google.com/run/docs/securing/using-cmek</rdfs:comment>
    <rdfs:domain rdf:resource="http://example.org/onto/class/google_cloud_run_v2_worker_pool"/>
    <rdfs:range rdf:resource="http://www.w3.org/2001/XMLSchema#string"/>
  </owl:DatatypeProperty>
  <owl:DatatypeProperty rdf:about="http://example.org/onto/prop/google_cloud_run_v2_worker_pool_encryption_key_revocation_action">
    <rdfs:label>encryption_key_revocation_action</rdfs:label>
    <rdfs:comment>The action to take if the encryption key is revoked. Possible values: ["PREVENT_NEW", "SHUTDOWN"]</rdfs:comment>
    <rdfs:domain rdf:resource="http://example.org/onto/class/google_cloud_run_v2_worker_pool"/>
    <rdfs:range rdf:resource="http://www.w3.org/2001/XMLSchema#string"/>
  </owl:DatatypeProperty>
  <owl:DatatypeProperty rdf:about="http://example.org/onto/prop/google_cloud_run_v2_worker_pool_encryption_key_shutdown_duration">
    <rdfs:label>encryption_key_shutdown_duration</rdfs:label>
    <rdfs:comment>If encryptionKeyRevocationAction is SHUTDOWN, the duration before shutting down all instances. The minimum increment is 1 hour.

A duration in seconds with up to nine fractional digits, ending with 's'. Example: "3.5s".</rdfs:comment>
    <rdfs:domain rdf:resource="http://example.org/onto/class/google_cloud_run_v2_worker_pool"/>
    <rdfs:range rdf:resource="http://www.w3.org/2001/XMLSchema#string"/>
  </owl:DatatypeProperty>
  <owl:DatatypeProperty rdf:about="http://example.org/onto/prop/google_cloud_run_v2_worker_pool_gpu_zonal_redundancy_disabled">
    <rdfs:label>gpu_zonal_redundancy_disabled</rdfs:label>
    <rdfs:comment>True if GPU zonal redundancy is disabled on this revision.</rdfs:comment>
    <rdfs:domain rdf:resource="http://example.org/onto/class/google_cloud_run_v2_worker_pool"/>
    <rdfs:range rdf:resource="http://www.w3.org/2001/XMLSchema#string"/>
  </owl:DatatypeProperty>
  <owl:DatatypeProperty rdf:about="http://example.org/onto/prop/google_cloud_run_v2_worker_pool_labels">
    <rdfs:label>labels</rdfs:label>
    <rdfs:comment>Unstructured key value map that can be used to organize and categorize objects. User-provided labels are shared with Google's billing system, so they can be used to filter, or break down billing charges by team, component, environment, state, etc.
For more information, visit https://cloud.google.com/resource-manager/docs/creating-managing-labels or https://cloud.google.com/run/docs/configuring/labels.

Cloud Run API v2 does not support labels with 'run.googleapis.com', 'cloud.googleapis.com', 'serving.knative.dev', or 'autoscaling.knative.dev' namespaces, and they will be rejected.
All system labels in v1 now have a corresponding field in v2 WorkerPoolRevisionTemplate.</rdfs:comment>
    <rdfs:domain rdf:resource="http://example.org/onto/class/google_cloud_run_v2_worker_pool"/>
    <rdfs:range rdf:resource="http://www.w3.org/2001/XMLSchema#string"/>
  </owl:DatatypeProperty>
  <owl:DatatypeProperty rdf:about="http://example.org/onto/prop/google_cloud_run_v2_worker_pool_revision">
    <rdfs:label>revision</rdfs:label>
    <rdfs:comment>The unique name for the revision. If this field is omitted, it will be automatically generated based on the WorkerPool name.</rdfs:comment>
    <rdfs:domain rdf:resource="http://example.org/onto/class/google_cloud_run_v2_worker_pool"/>
    <rdfs:range rdf:resource="http://www.w3.org/2001/XMLSchema#string"/>
  </owl:DatatypeProperty>
  <owl:DatatypeProperty rdf:about="http://example.org/onto/prop/google_cloud_run_v2_worker_pool_service_account">
    <rdfs:label>service_account</rdfs:label>
    <rdfs:comment>Email address of the IAM service account associated with the revision of the WorkerPool. The service account represents the identity of the running revision, and determines what permissions the revision has. If not provided, the revision will use the project's default service account.</rdfs:comment>
    <rdfs:domain rdf:resource="http://example.org/onto/class/google_cloud_run_v2_worker_pool"/>
    <rdfs:range rdf:resource="http://www.w3.org/2001/XMLSchema#string"/>
  </owl:DatatypeProperty>
  <owl:DatatypeProperty rdf:about="http://example.org/onto/prop/google_cloud_run_v2_worker_pool_args">
    <rdfs:label>args</rdfs:label>
    <rdfs:comment>Arguments to the entrypoint. The docker image's CMD is used if this is not provided. Variable references are not supported in Cloud Run.</rdfs:comment>
    <rdfs:domain rdf:resource="http://example.org/onto/class/google_cloud_run_v2_worker_pool"/>
    <rdfs:range rdf:resource="http://www.w3.org/2001/XMLSchema#string"/>
  </owl:DatatypeProperty>
  <owl:DatatypeProperty rdf:about="http://example.org/onto/prop/google_cloud_run_v2_worker_pool_command">
    <rdfs:label>command</rdfs:label>
    <rdfs:comment>Entrypoint array. Not executed within a shell. The docker image's ENTRYPOINT is used if this is not provided. Variable references $(VAR_NAME) are expanded using the container's environment. If a variable cannot be resolved, the reference in the input string will be unchanged. The $(VAR_NAME) syntax can be escaped with a double $$, ie: $$(VAR_NAME). Escaped references will never be expanded, regardless of whether the variable exists or not. More info: https://kubernetes.io/docs/tasks/inject-data-application/define-command-argument-container/#running-a-command-in-a-shell</rdfs:comment>
    <rdfs:domain rdf:resource="http://example.org/onto/class/google_cloud_run_v2_worker_pool"/>
    <rdfs:range rdf:resource="http://www.w3.org/2001/XMLSchema#string"/>
  </owl:DatatypeProperty>
  <owl:DatatypeProperty rdf:about="http://example.org/onto/prop/google_cloud_run_v2_worker_pool_image">
    <rdfs:label>image</rdfs:label>
    <rdfs:comment>URL of the Container image in Google Container Registry or Google Artifact Registry. More info: https://kubernetes.io/docs/concepts/containers/images</rdfs:comment>
    <rdfs:domain rdf:resource="http://example.org/onto/class/google_cloud_run_v2_worker_pool"/>
    <rdfs:range rdf:resource="http://www.w3.org/2001/XMLSchema#string"/>
  </owl:DatatypeProperty>
  <owl:DatatypeProperty rdf:about="http://example.org/onto/prop/google_cloud_run_v2_worker_pool_name">
    <rdfs:label>name</rdfs:label>
    <rdfs:comment>Name of the container specified as a DNS_LABEL.</rdfs:comment>
    <rdfs:domain rdf:resource="http://example.org/onto/class/google_cloud_run_v2_worker_pool"/>
    <rdfs:range rdf:resource="http://www.w3.org/2001/XMLSchema#string"/>
  </owl:DatatypeProperty>
  <owl:DatatypeProperty rdf:about="http://example.org/onto/prop/google_cloud_run_v2_worker_pool_working_dir">
    <rdfs:label>working_dir</rdfs:label>
    <rdfs:comment>Container's working directory. If not specified, the container runtime's default will be used, which might be configured in the container image.</rdfs:comment>
    <rdfs:domain rdf:resource="http://example.org/onto/class/google_cloud_run_v2_worker_pool"/>
    <rdfs:range rdf:resource="http://www.w3.org/2001/XMLSchema#string"/>
  </owl:DatatypeProperty>
  <owl:DatatypeProperty rdf:about="http://example.org/onto/prop/google_cloud_run_v2_worker_pool_name">
    <rdfs:label>name</rdfs:label>
    <rdfs:comment>Name of the environment variable. Must be a C_IDENTIFIER, and may not exceed 32768 characters.</rdfs:comment>
    <rdfs:domain rdf:resource="http://example.org/onto/class/google_cloud_run_v2_worker_pool"/>
    <rdfs:range rdf:resource="http://www.w3.org/2001/XMLSchema#string"/>
  </owl:DatatypeProperty>
  <owl:DatatypeProperty rdf:about="http://example.org/onto/prop/google_cloud_run_v2_worker_pool_value">
    <rdfs:label>value</rdfs:label>
    <rdfs:comment>Literal value of the environment variable. Defaults to "" and the maximum allowed length is 32768 characters. Variable references are not supported in Cloud Run.</rdfs:comment>
    <rdfs:domain rdf:resource="http://example.org/onto/class/google_cloud_run_v2_worker_pool"/>
    <rdfs:range rdf:resource="http://www.w3.org/2001/XMLSchema#string"/>
  </owl:DatatypeProperty>
  <owl:DatatypeProperty rdf:about="http://example.org/onto/prop/google_cloud_run_v2_worker_pool_secret">
    <rdfs:label>secret</rdfs:label>
    <rdfs:comment>The name of the secret in Cloud Secret Manager. Format: {secretName} if the secret is in the same project. projects/{project}/secrets/{secretName} if the secret is in a different project.</rdfs:comment>
    <rdfs:domain rdf:resource="http://example.org/onto/class/google_cloud_run_v2_worker_pool"/>
    <rdfs:range rdf:resource="http://www.w3.org/2001/XMLSchema#string"/>
  </owl:DatatypeProperty>
  <owl:DatatypeProperty rdf:about="http://example.org/onto/prop/google_cloud_run_v2_worker_pool_version">
    <rdfs:label>version</rdfs:label>
    <rdfs:comment>The Cloud Secret Manager secret version. Can be 'latest' for the latest value or an integer for a specific version.</rdfs:comment>
    <rdfs:domain rdf:resource="http://example.org/onto/class/google_cloud_run_v2_worker_pool"/>
    <rdfs:range rdf:resource="http://www.w3.org/2001/XMLSchema#string"/>
  </owl:DatatypeProperty>
  <owl:DatatypeProperty rdf:about="http://example.org/onto/prop/google_cloud_run_v2_worker_pool_failure_threshold">
    <rdfs:label>failure_threshold</rdfs:label>
    <rdfs:comment>Optional. Minimum consecutive failures for the probe to be considered failed after having succeeded. Defaults to 3. Minimum value is 1.</rdfs:comment>
    <rdfs:domain rdf:resource="http://example.org/onto/class/google_cloud_run_v2_worker_pool"/>
    <rdfs:range rdf:resource="http://www.w3.org/2001/XMLSchema#string"/>
  </owl:DatatypeProperty>
  <owl:DatatypeProperty rdf:about="http://example.org/onto/prop/google_cloud_run_v2_worker_pool_initial_delay_seconds">
    <rdfs:label>initial_delay_seconds</rdfs:label>
    <rdfs:comment>Optional. Number of seconds after the container has started before the probe is initiated. Defaults to 0 seconds. Minimum value is 0. Maximum value for liveness probe is 3600. Maximum value for startup probe is 240.</rdfs:comment>
    <rdfs:domain rdf:resource="http://example.org/onto/class/google_cloud_run_v2_worker_pool"/>
    <rdfs:range rdf:resource="http://www.w3.org/2001/XMLSchema#string"/>
  </owl:DatatypeProperty>
  <owl:DatatypeProperty rdf:about="http://example.org/onto/prop/google_cloud_run_v2_worker_pool_period_seconds">
    <rdfs:label>period_seconds</rdfs:label>
    <rdfs:comment>Optional. How often (in seconds) to perform the probe. Default to 10 seconds. Minimum value is 1. Maximum value for liveness probe is 3600. Maximum value for startup probe is 240. Must be greater or equal than timeout_seconds.</rdfs:comment>
    <rdfs:domain rdf:resource="http://example.org/onto/class/google_cloud_run_v2_worker_pool"/>
    <rdfs:range rdf:resource="http://www.w3.org/2001/XMLSchema#string"/>
  </owl:DatatypeProperty>
  <owl:DatatypeProperty rdf:about="http://example.org/onto/prop/google_cloud_run_v2_worker_pool_timeout_seconds">
    <rdfs:label>timeout_seconds</rdfs:label>
    <rdfs:comment>Optional. Number of seconds after which the probe times out. Defaults to 1 second. Minimum value is 1. Maximum value is 3600. Must be smaller than period_seconds.</rdfs:comment>
    <rdfs:domain rdf:resource="http://example.org/onto/class/google_cloud_run_v2_worker_pool"/>
    <rdfs:range rdf:resource="http://www.w3.org/2001/XMLSchema#string"/>
  </owl:DatatypeProperty>
  <owl:DatatypeProperty rdf:about="http://example.org/onto/prop/google_cloud_run_v2_worker_pool_port">
    <rdfs:label>port</rdfs:label>
    <rdfs:comment>Optional. Port number of the gRPC service. Number must be in the range 1 to 65535. If not specified, defaults to the exposed port of the container, which is the value of container.ports[0].containerPort.</rdfs:comment>
    <rdfs:domain rdf:resource="http://example.org/onto/class/google_cloud_run_v2_worker_pool"/>
    <rdfs:range rdf:resource="http://www.w3.org/2001/XMLSchema#string"/>
  </owl:DatatypeProperty>
  <owl:DatatypeProperty rdf:about="http://example.org/onto/prop/google_cloud_run_v2_worker_pool_service">
    <rdfs:label>service</rdfs:label>
    <rdfs:comment>Optional. Service is the name of the service to place in the gRPC HealthCheckRequest (see https://github.com/grpc/grpc/blob/master/doc/health-checking.md ). If this is not specified, the default behavior is defined by gRPC</rdfs:comment>
    <rdfs:domain rdf:resource="http://example.org/onto/class/google_cloud_run_v2_worker_pool"/>
    <rdfs:range rdf:resource="http://www.w3.org/2001/XMLSchema#string"/>
  </owl:DatatypeProperty>
  <owl:DatatypeProperty rdf:about="http://example.org/onto/prop/google_cloud_run_v2_worker_pool_path">
    <rdfs:label>path</rdfs:label>
    <rdfs:comment>Optional. Path to access on the HTTP server. Defaults to '/'.</rdfs:comment>
    <rdfs:domain rdf:resource="http://example.org/onto/class/google_cloud_run_v2_worker_pool"/>
    <rdfs:range rdf:resource="http://www.w3.org/2001/XMLSchema#string"/>
  </owl:DatatypeProperty>
  <owl:DatatypeProperty rdf:about="http://example.org/onto/prop/google_cloud_run_v2_worker_pool_port">
    <rdfs:label>port</rdfs:label>
    <rdfs:comment>Optional. Port number to access on the container. Must be in the range 1 to 65535. If not specified, defaults to the exposed port of the container, which is the value of container.ports[0].containerPort.</rdfs:comment>
    <rdfs:domain rdf:resource="http://example.org/onto/class/google_cloud_run_v2_worker_pool"/>
    <rdfs:range rdf:resource="http://www.w3.org/2001/XMLSchema#string"/>
  </owl:DatatypeProperty>
  <owl:DatatypeProperty rdf:about="http://example.org/onto/prop/google_cloud_run_v2_worker_pool_port">
    <rdfs:label>port</rdfs:label>
    <rdfs:comment>Required. The header field name</rdfs:comment>
    <rdfs:domain rdf:resource="http://example.org/onto/class/google_cloud_run_v2_worker_pool"/>
    <rdfs:range rdf:resource="http://www.w3.org/2001/XMLSchema#string"/>
  </owl:DatatypeProperty>
  <owl:DatatypeProperty rdf:about="http://example.org/onto/prop/google_cloud_run_v2_worker_pool_value">
    <rdfs:label>value</rdfs:label>
    <rdfs:comment>Optional. The header field value</rdfs:comment>
    <rdfs:domain rdf:resource="http://example.org/onto/class/google_cloud_run_v2_worker_pool"/>
    <rdfs:range rdf:resource="http://www.w3.org/2001/XMLSchema#string"/>
  </owl:DatatypeProperty>
  <owl:DatatypeProperty rdf:about="http://example.org/onto/prop/google_cloud_run_v2_worker_pool_port">
    <rdfs:label>port</rdfs:label>
    <rdfs:comment>Optional. Port number to access on the container. Must be in the range 1 to 65535. If not specified, defaults to the exposed port of the container, which is the value of container.ports[0].containerPort.</rdfs:comment>
    <rdfs:domain rdf:resource="http://example.org/onto/class/google_cloud_run_v2_worker_pool"/>
    <rdfs:range rdf:resource="http://www.w3.org/2001/XMLSchema#string"/>
  </owl:DatatypeProperty>
  <owl:DatatypeProperty rdf:about="http://example.org/onto/prop/google_cloud_run_v2_worker_pool_limits">
    <rdfs:label>limits</rdfs:label>
    <rdfs:comment>Only memory, CPU, and nvidia.com/gpu are supported. Use key 'cpu' for CPU limit, 'memory' for memory limit, 'nvidia.com/gpu' for gpu limit. Note: The only supported values for CPU are '1', '2', '4', and '8'. Setting 4 CPU requires at least 2Gi of memory. The values of the map is string form of the 'quantity' k8s type: https://github.com/kubernetes/kubernetes/blob/master/staging/src/k8s.io/apimachinery/pkg/api/resource/quantity.go</rdfs:comment>
    <rdfs:domain rdf:resource="http://example.org/onto/class/google_cloud_run_v2_worker_pool"/>
    <rdfs:range rdf:resource="http://www.w3.org/2001/XMLSchema#string"/>
  </owl:DatatypeProperty>
  <owl:DatatypeProperty rdf:about="http://example.org/onto/prop/google_cloud_run_v2_worker_pool_failure_threshold">
    <rdfs:label>failure_threshold</rdfs:label>
    <rdfs:comment>Optional. Minimum consecutive failures for the probe to be considered failed after having succeeded. Defaults to 3. Minimum value is 1.</rdfs:comment>
    <rdfs:domain rdf:resource="http://example.org/onto/class/google_cloud_run_v2_worker_pool"/>
    <rdfs:range rdf:resource="http://www.w3.org/2001/XMLSchema#string"/>
  </owl:DatatypeProperty>
  <owl:DatatypeProperty rdf:about="http://example.org/onto/prop/google_cloud_run_v2_worker_pool_initial_delay_seconds">
    <rdfs:label>initial_delay_seconds</rdfs:label>
    <rdfs:comment>Optional. Number of seconds after the container has started before the probe is initiated. Defaults to 0 seconds. Minimum value is 0. Maximum value for liveness probe is 3600. Maximum value for startup probe is 240.</rdfs:comment>
    <rdfs:domain rdf:resource="http://example.org/onto/class/google_cloud_run_v2_worker_pool"/>
    <rdfs:range rdf:resource="http://www.w3.org/2001/XMLSchema#string"/>
  </owl:DatatypeProperty>
  <owl:DatatypeProperty rdf:about="http://example.org/onto/prop/google_cloud_run_v2_worker_pool_period_seconds">
    <rdfs:label>period_seconds</rdfs:label>
    <rdfs:comment>Optional. How often (in seconds) to perform the probe. Default to 10 seconds. Minimum value is 1. Maximum value for liveness probe is 3600. Maximum value for startup probe is 240. Must be greater or equal than timeout_seconds.</rdfs:comment>
    <rdfs:domain rdf:resource="http://example.org/onto/class/google_cloud_run_v2_worker_pool"/>
    <rdfs:range rdf:resource="http://www.w3.org/2001/XMLSchema#string"/>
  </owl:DatatypeProperty>
  <owl:DatatypeProperty rdf:about="http://example.org/onto/prop/google_cloud_run_v2_worker_pool_timeout_seconds">
    <rdfs:label>timeout_seconds</rdfs:label>
    <rdfs:comment>Optional. Number of seconds after which the probe times out. Defaults to 1 second. Minimum value is 1. Maximum value is 3600. Must be smaller than period_seconds.</rdfs:comment>
    <rdfs:domain rdf:resource="http://example.org/onto/class/google_cloud_run_v2_worker_pool"/>
    <rdfs:range rdf:resource="http://www.w3.org/2001/XMLSchema#string"/>
  </owl:DatatypeProperty>
  <owl:DatatypeProperty rdf:about="http://example.org/onto/prop/google_cloud_run_v2_worker_pool_port">
    <rdfs:label>port</rdfs:label>
    <rdfs:comment>Optional. Port number of the gRPC service. Number must be in the range 1 to 65535. If not specified, defaults to the exposed port of the container, which is the value of container.ports[0].containerPort.</rdfs:comment>
    <rdfs:domain rdf:resource="http://example.org/onto/class/google_cloud_run_v2_worker_pool"/>
    <rdfs:range rdf:resource="http://www.w3.org/2001/XMLSchema#string"/>
  </owl:DatatypeProperty>
  <owl:DatatypeProperty rdf:about="http://example.org/onto/prop/google_cloud_run_v2_worker_pool_service">
    <rdfs:label>service</rdfs:label>
    <rdfs:comment>Optional. Service is the name of the service to place in the gRPC HealthCheckRequest (see https://github.com/grpc/grpc/blob/master/doc/health-checking.md ). If this is not specified, the default behavior is defined by gRPC</rdfs:comment>
    <rdfs:domain rdf:resource="http://example.org/onto/class/google_cloud_run_v2_worker_pool"/>
    <rdfs:range rdf:resource="http://www.w3.org/2001/XMLSchema#string"/>
  </owl:DatatypeProperty>
  <owl:DatatypeProperty rdf:about="http://example.org/onto/prop/google_cloud_run_v2_worker_pool_path">
    <rdfs:label>path</rdfs:label>
    <rdfs:comment>Optional. Path to access on the HTTP server. Defaults to '/'.</rdfs:comment>
    <rdfs:domain rdf:resource="http://example.org/onto/class/google_cloud_run_v2_worker_pool"/>
    <rdfs:range rdf:resource="http://www.w3.org/2001/XMLSchema#string"/>
  </owl:DatatypeProperty>
  <owl:DatatypeProperty rdf:about="http://example.org/onto/prop/google_cloud_run_v2_worker_pool_port">
    <rdfs:label>port</rdfs:label>
    <rdfs:comment>Optional. Port number to access on the container. Must be in the range 1 to 65535. If not specified, defaults to the exposed port of the container, which is the value of container.ports[0].containerPort.</rdfs:comment>
    <rdfs:domain rdf:resource="http://example.org/onto/class/google_cloud_run_v2_worker_pool"/>
    <rdfs:range rdf:resource="http://www.w3.org/2001/XMLSchema#string"/>
  </owl:DatatypeProperty>
  <owl:DatatypeProperty rdf:about="http://example.org/onto/prop/google_cloud_run_v2_worker_pool_port">
    <rdfs:label>port</rdfs:label>
    <rdfs:comment>Required. The header field name</rdfs:comment>
    <rdfs:domain rdf:resource="http://example.org/onto/class/google_cloud_run_v2_worker_pool"/>
    <rdfs:range rdf:resource="http://www.w3.org/2001/XMLSchema#string"/>
  </owl:DatatypeProperty>
  <owl:DatatypeProperty rdf:about="http://example.org/onto/prop/google_cloud_run_v2_worker_pool_value">
    <rdfs:label>value</rdfs:label>
    <rdfs:comment>Optional. The header field value</rdfs:comment>
    <rdfs:domain rdf:resource="http://example.org/onto/class/google_cloud_run_v2_worker_pool"/>
    <rdfs:range rdf:resource="http://www.w3.org/2001/XMLSchema#string"/>
  </owl:DatatypeProperty>
  <owl:DatatypeProperty rdf:about="http://example.org/onto/prop/google_cloud_run_v2_worker_pool_port">
    <rdfs:label>port</rdfs:label>
    <rdfs:comment>Optional. Port number to access on the container. Must be in the range 1 to 65535. If not specified, defaults to the exposed port of the container, which is the value of container.ports[0].containerPort.</rdfs:comment>
    <rdfs:domain rdf:resource="http://example.org/onto/class/google_cloud_run_v2_worker_pool"/>
    <rdfs:range rdf:resource="http://www.w3.org/2001/XMLSchema#string"/>
  </owl:DatatypeProperty>
  <owl:DatatypeProperty rdf:about="http://example.org/onto/prop/google_cloud_run_v2_worker_pool_mount_path">
    <rdfs:label>mount_path</rdfs:label>
    <rdfs:comment>Path within the container at which the volume should be mounted. Must not contain ':'. For Cloud SQL volumes, it can be left empty, or must otherwise be /cloudsql. All instances defined in the Volume will be available as /cloudsql/[instance]. For more information on Cloud SQL volumes, visit https://cloud.google.com/sql/docs/mysql/connect-run</rdfs:comment>
    <rdfs:domain rdf:resource="http://example.org/onto/class/google_cloud_run_v2_worker_pool"/>
    <rdfs:range rdf:resource="http://www.w3.org/2001/XMLSchema#string"/>
  </owl:DatatypeProperty>
  <owl:DatatypeProperty rdf:about="http://example.org/onto/prop/google_cloud_run_v2_worker_pool_name">
    <rdfs:label>name</rdfs:label>
    <rdfs:comment>This must match the Name of a Volume.</rdfs:comment>
    <rdfs:domain rdf:resource="http://example.org/onto/class/google_cloud_run_v2_worker_pool"/>
    <rdfs:range rdf:resource="http://www.w3.org/2001/XMLSchema#string"/>
  </owl:DatatypeProperty>
  <owl:DatatypeProperty rdf:about="http://example.org/onto/prop/google_cloud_run_v2_worker_pool_sub_path">
    <rdfs:label>sub_path</rdfs:label>
    <rdfs:comment>Path within the volume from which the container's volume should be mounted.</rdfs:comment>
    <rdfs:domain rdf:resource="http://example.org/onto/class/google_cloud_run_v2_worker_pool"/>
    <rdfs:range rdf:resource="http://www.w3.org/2001/XMLSchema#string"/>
  </owl:DatatypeProperty>
  <owl:DatatypeProperty rdf:about="http://example.org/onto/prop/google_cloud_run_v2_worker_pool_accelerator">
    <rdfs:label>accelerator</rdfs:label>
    <rdfs:comment>The GPU to attach to an instance. See https://cloud.google.com/run/docs/configuring/services/gpu for configuring GPU.</rdfs:comment>
    <rdfs:domain rdf:resource="http://example.org/onto/class/google_cloud_run_v2_worker_pool"/>
    <rdfs:range rdf:resource="http://www.w3.org/2001/XMLSchema#string"/>
  </owl:DatatypeProperty>
  <owl:DatatypeProperty rdf:about="http://example.org/onto/prop/google_cloud_run_v2_worker_pool_name">
    <rdfs:label>name</rdfs:label>
    <rdfs:comment>Volume's name.</rdfs:comment>
    <rdfs:domain rdf:resource="http://example.org/onto/class/google_cloud_run_v2_worker_pool"/>
    <rdfs:range rdf:resource="http://www.w3.org/2001/XMLSchema#string"/>
  </owl:DatatypeProperty>
  <owl:DatatypeProperty rdf:about="http://example.org/onto/prop/google_cloud_run_v2_worker_pool_instances">
    <rdfs:label>instances</rdfs:label>
    <rdfs:comment>The Cloud SQL instance connection names, as can be found in https://console.cloud.google.com/sql/instances. Visit https://cloud.google.com/sql/docs/mysql/connect-run for more information on how to connect Cloud SQL and Cloud Run. Format: {project}:{location}:{instance}</rdfs:comment>
    <rdfs:domain rdf:resource="http://example.org/onto/class/google_cloud_run_v2_worker_pool"/>
    <rdfs:range rdf:resource="http://www.w3.org/2001/XMLSchema#string"/>
  </owl:DatatypeProperty>
  <owl:DatatypeProperty rdf:about="http://example.org/onto/prop/google_cloud_run_v2_worker_pool_medium">
    <rdfs:label>medium</rdfs:label>
    <rdfs:comment>The different types of medium supported for EmptyDir. Default value: "MEMORY" Possible values: ["MEMORY"]</rdfs:comment>
    <rdfs:domain rdf:resource="http://example.org/onto/class/google_cloud_run_v2_worker_pool"/>
    <rdfs:range rdf:resource="http://www.w3.org/2001/XMLSchema#string"/>
  </owl:DatatypeProperty>
  <owl:DatatypeProperty rdf:about="http://example.org/onto/prop/google_cloud_run_v2_worker_pool_size_limit">
    <rdfs:label>size_limit</rdfs:label>
    <rdfs:comment>Limit on the storage usable by this EmptyDir volume. The size limit is also applicable for memory medium. The maximum usage on memory medium EmptyDir would be the minimum value between the SizeLimit specified here and the sum of memory limits of all containers in a pod. This field's values are of the 'Quantity' k8s type: https://kubernetes.io/docs/reference/kubernetes-api/common-definitions/quantity/. The default is nil which means that the limit is undefined. More info: https://kubernetes.io/docs/concepts/storage/volumes/#emptydir.</rdfs:comment>
    <rdfs:domain rdf:resource="http://example.org/onto/class/google_cloud_run_v2_worker_pool"/>
    <rdfs:range rdf:resource="http://www.w3.org/2001/XMLSchema#string"/>
  </owl:DatatypeProperty>
  <owl:DatatypeProperty rdf:about="http://example.org/onto/prop/google_cloud_run_v2_worker_pool_bucket">
    <rdfs:label>bucket</rdfs:label>
    <rdfs:comment>GCS Bucket name</rdfs:comment>
    <rdfs:domain rdf:resource="http://example.org/onto/class/google_cloud_run_v2_worker_pool"/>
    <rdfs:range rdf:resource="http://www.w3.org/2001/XMLSchema#string"/>
  </owl:DatatypeProperty>
  <owl:DatatypeProperty rdf:about="http://example.org/onto/prop/google_cloud_run_v2_worker_pool_mount_options">
    <rdfs:label>mount_options</rdfs:label>
    <rdfs:comment>A list of flags to pass to the gcsfuse command for configuring this volume.
Flags should be passed without leading dashes.</rdfs:comment>
    <rdfs:domain rdf:resource="http://example.org/onto/class/google_cloud_run_v2_worker_pool"/>
    <rdfs:range rdf:resource="http://www.w3.org/2001/XMLSchema#string"/>
  </owl:DatatypeProperty>
  <owl:DatatypeProperty rdf:about="http://example.org/onto/prop/google_cloud_run_v2_worker_pool_read_only">
    <rdfs:label>read_only</rdfs:label>
    <rdfs:comment>If true, mount the GCS bucket as read-only</rdfs:comment>
    <rdfs:domain rdf:resource="http://example.org/onto/class/google_cloud_run_v2_worker_pool"/>
    <rdfs:range rdf:resource="http://www.w3.org/2001/XMLSchema#string"/>
  </owl:DatatypeProperty>
  <owl:DatatypeProperty rdf:about="http://example.org/onto/prop/google_cloud_run_v2_worker_pool_path">
    <rdfs:label>path</rdfs:label>
    <rdfs:comment>Path that is exported by the NFS server.</rdfs:comment>
    <rdfs:domain rdf:resource="http://example.org/onto/class/google_cloud_run_v2_worker_pool"/>
    <rdfs:range rdf:resource="http://www.w3.org/2001/XMLSchema#string"/>
  </owl:DatatypeProperty>
  <owl:DatatypeProperty rdf:about="http://example.org/onto/prop/google_cloud_run_v2_worker_pool_read_only">
    <rdfs:label>read_only</rdfs:label>
    <rdfs:comment>If true, mount the NFS volume as read only</rdfs:comment>
    <rdfs:domain rdf:resource="http://example.org/onto/class/google_cloud_run_v2_worker_pool"/>
    <rdfs:range rdf:resource="http://www.w3.org/2001/XMLSchema#string"/>
  </owl:DatatypeProperty>
  <owl:DatatypeProperty rdf:about="http://example.org/onto/prop/google_cloud_run_v2_worker_pool_server">
    <rdfs:label>server</rdfs:label>
    <rdfs:comment>Hostname or IP address of the NFS server</rdfs:comment>
    <rdfs:domain rdf:resource="http://example.org/onto/class/google_cloud_run_v2_worker_pool"/>
    <rdfs:range rdf:resource="http://www.w3.org/2001/XMLSchema#string"/>
  </owl:DatatypeProperty>
  <owl:DatatypeProperty rdf:about="http://example.org/onto/prop/google_cloud_run_v2_worker_pool_default_mode">
    <rdfs:label>default_mode</rdfs:label>
    <rdfs:comment>Integer representation of mode bits to use on created files by default. Must be a value between 0000 and 0777 (octal), defaulting to 0444. Directories within the path are not affected by this setting.</rdfs:comment>
    <rdfs:domain rdf:resource="http://example.org/onto/class/google_cloud_run_v2_worker_pool"/>
    <rdfs:range rdf:resource="http://www.w3.org/2001/XMLSchema#string"/>
  </owl:DatatypeProperty>
  <owl:DatatypeProperty rdf:about="http://example.org/onto/prop/google_cloud_run_v2_worker_pool_secret">
    <rdfs:label>secret</rdfs:label>
    <rdfs:comment>The name of the secret in Cloud Secret Manager. Format: {secret} if the secret is in the same project. projects/{project}/secrets/{secret} if the secret is in a different project.</rdfs:comment>
    <rdfs:domain rdf:resource="http://example.org/onto/class/google_cloud_run_v2_worker_pool"/>
    <rdfs:range rdf:resource="http://www.w3.org/2001/XMLSchema#string"/>
  </owl:DatatypeProperty>
  <owl:DatatypeProperty rdf:about="http://example.org/onto/prop/google_cloud_run_v2_worker_pool_mode">
    <rdfs:label>mode</rdfs:label>
    <rdfs:comment>Integer octal mode bits to use on this file, must be a value between 01 and 0777 (octal). If 0 or not set, the Volume's default mode will be used.</rdfs:comment>
    <rdfs:domain rdf:resource="http://example.org/onto/class/google_cloud_run_v2_worker_pool"/>
    <rdfs:range rdf:resource="http://www.w3.org/2001/XMLSchema#string"/>
  </owl:DatatypeProperty>
  <owl:DatatypeProperty rdf:about="http://example.org/onto/prop/google_cloud_run_v2_worker_pool_path">
    <rdfs:label>path</rdfs:label>
    <rdfs:comment>The relative path of the secret in the container.</rdfs:comment>
    <rdfs:domain rdf:resource="http://example.org/onto/class/google_cloud_run_v2_worker_pool"/>
    <rdfs:range rdf:resource="http://www.w3.org/2001/XMLSchema#string"/>
  </owl:DatatypeProperty>
  <owl:DatatypeProperty rdf:about="http://example.org/onto/prop/google_cloud_run_v2_worker_pool_version">
    <rdfs:label>version</rdfs:label>
    <rdfs:comment>The Cloud Secret Manager secret version. Can be 'latest' for the latest value or an integer for a specific version</rdfs:comment>
    <rdfs:domain rdf:resource="http://example.org/onto/class/google_cloud_run_v2_worker_pool"/>
    <rdfs:range rdf:resource="http://www.w3.org/2001/XMLSchema#string"/>
  </owl:DatatypeProperty>
  <owl:DatatypeProperty rdf:about="http://example.org/onto/prop/google_cloud_run_v2_worker_pool_connector">
    <rdfs:label>connector</rdfs:label>
    <rdfs:comment>VPC Access connector name. Format: projects/{project}/locations/{location}/connectors/{connector}, where {project} can be project id or number.</rdfs:comment>
    <rdfs:domain rdf:resource="http://example.org/onto/class/google_cloud_run_v2_worker_pool"/>
    <rdfs:range rdf:resource="http://www.w3.org/2001/XMLSchema#string"/>
  </owl:DatatypeProperty>
  <owl:DatatypeProperty rdf:about="http://example.org/onto/prop/google_cloud_run_v2_worker_pool_egress">
    <rdfs:label>egress</rdfs:label>
    <rdfs:comment>Traffic VPC egress settings. Possible values: ["ALL_TRAFFIC", "PRIVATE_RANGES_ONLY"]</rdfs:comment>
    <rdfs:domain rdf:resource="http://example.org/onto/class/google_cloud_run_v2_worker_pool"/>
    <rdfs:range rdf:resource="http://www.w3.org/2001/XMLSchema#string"/>
  </owl:DatatypeProperty>
  <owl:DatatypeProperty rdf:about="http://example.org/onto/prop/google_cloud_run_v2_worker_pool_network">
    <rdfs:label>network</rdfs:label>
    <rdfs:comment>The VPC network that the Cloud Run resource will be able to send traffic to. At least one of network or subnetwork must be specified. If both
network and subnetwork are specified, the given VPC subnetwork must belong to the given VPC network. If network is not specified, it will be
looked up from the subnetwork.</rdfs:comment>
    <rdfs:domain rdf:resource="http://example.org/onto/class/google_cloud_run_v2_worker_pool"/>
    <rdfs:range rdf:resource="http://www.w3.org/2001/XMLSchema#string"/>
  </owl:DatatypeProperty>
  <owl:DatatypeProperty rdf:about="http://example.org/onto/prop/google_cloud_run_v2_worker_pool_subnetwork">
    <rdfs:label>subnetwork</rdfs:label>
    <rdfs:comment>The VPC subnetwork that the Cloud Run resource will get IPs from. At least one of network or subnetwork must be specified. If both
network and subnetwork are specified, the given VPC subnetwork must belong to the given VPC network. If subnetwork is not specified, the
subnetwork with the same name with the network will be used.</rdfs:comment>
    <rdfs:domain rdf:resource="http://example.org/onto/class/google_cloud_run_v2_worker_pool"/>
    <rdfs:range rdf:resource="http://www.w3.org/2001/XMLSchema#string"/>
  </owl:DatatypeProperty>
  <owl:DatatypeProperty rdf:about="http://example.org/onto/prop/google_cloud_run_v2_worker_pool_tags">
    <rdfs:label>tags</rdfs:label>
    <rdfs:comment>Network tags applied to this Cloud Run WorkerPool.</rdfs:comment>
    <rdfs:domain rdf:resource="http://example.org/onto/class/google_cloud_run_v2_worker_pool"/>
    <rdfs:range rdf:resource="http://www.w3.org/2001/XMLSchema#string"/>
  </owl:DatatypeProperty>
  <owl:DatatypeProperty rdf:about="http://example.org/onto/prop/google_cloud_run_v2_worker_pool_create">
    <rdfs:label>create</rdfs:label>
    <rdfs:domain rdf:resource="http://example.org/onto/class/google_cloud_run_v2_worker_pool"/>
    <rdfs:range rdf:resource="http://www.w3.org/2001/XMLSchema#string"/>
  </owl:DatatypeProperty>
  <owl:DatatypeProperty rdf:about="http://example.org/onto/prop/google_cloud_run_v2_worker_pool_delete">
    <rdfs:label>delete</rdfs:label>
    <rdfs:domain rdf:resource="http://example.org/onto/class/google_cloud_run_v2_worker_pool"/>
    <rdfs:range rdf:resource="http://www.w3.org/2001/XMLSchema#string"/>
  </owl:DatatypeProperty>
  <owl:DatatypeProperty rdf:about="http://example.org/onto/prop/google_cloud_run_v2_worker_pool_update">
    <rdfs:label>update</rdfs:label>
    <rdfs:domain rdf:resource="http://example.org/onto/class/google_cloud_run_v2_worker_pool"/>
    <rdfs:range rdf:resource="http://www.w3.org/2001/XMLSchema#string"/>
  </owl:DatatypeProperty>
</rdf:RDF>
