<?xml version="1.0" encoding="UTF-8"?>
<rdf:RDF
  xmlns:rdf="http://www.w3.org/1999/02/22-rdf-syntax-ns#"
  xmlns:rdfs="http://www.w3.org/2000/01/rdf-schema#"
  xmlns:owl="http://www.w3.org/2002/07/owl#"
  xmlns:xsd="http://www.w3.org/2001/XMLSchema#"
  xml:base="http://example.org/onto/">
  <owl:Class rdf:about="http://example.org/onto/class/google_workflows_workflow">
    <rdfs:label>google_workflows_workflow</rdfs:label>
    <rdfs:comment>#
#     ***     AUTO GENERATED CODE    ***    Type: MMv1     ***
#
# ----------------------------------------------------------------------------
#
#     This code is generated by Magic Modules using the following:
#
#     Configuration: https:#github.com/GoogleCloudPlatform/magic-modules/tree/main/mmv1/products/workflows/Workflow.yaml
#     Template:      https:#github.com/GoogleCloudPlatform/magic-modules/tree/main/mmv1/templates/terraform/resource.html.markdown.tmpl
#
#     DO NOT EDIT this file directly. Any changes made to this file will be
#     overwritten during the next generation cycle.
#
# ----------------------------------------------------------------------------
subcategory: "Workflows"
description: |-
  Workflow program to be executed by Workflows.
---</rdfs:comment>
  </owl:Class>
  <owl:DatatypeProperty rdf:about="http://example.org/onto/prop/google_workflows_workflow_call_log_level">
    <rdfs:label>call_log_level</rdfs:label>
    <rdfs:comment>Describes the level of platform logging to apply to calls and call responses during
executions of this workflow. If both the workflow and the execution specify a logging level,
the execution level takes precedence. Possible values: ["CALL_LOG_LEVEL_UNSPECIFIED", "LOG_ALL_CALLS", "LOG_ERRORS_ONLY", "LOG_NONE"]</rdfs:comment>
    <rdfs:domain rdf:resource="http://example.org/onto/class/google_workflows_workflow"/>
    <rdfs:range rdf:resource="http://www.w3.org/2001/XMLSchema#string"/>
  </owl:DatatypeProperty>
  <owl:DatatypeProperty rdf:about="http://example.org/onto/prop/google_workflows_workflow_create_time">
    <rdfs:label>create_time</rdfs:label>
    <rdfs:comment>The timestamp of when the workflow was created in RFC3339 UTC "Zulu" format, with nanosecond resolution and up to nine fractional digits.</rdfs:comment>
    <rdfs:domain rdf:resource="http://example.org/onto/class/google_workflows_workflow"/>
    <rdfs:range rdf:resource="http://www.w3.org/2001/XMLSchema#string"/>
  </owl:DatatypeProperty>
  <owl:DatatypeProperty rdf:about="http://example.org/onto/prop/google_workflows_workflow_crypto_key_name">
    <rdfs:label>crypto_key_name</rdfs:label>
    <rdfs:comment>The KMS key used to encrypt workflow and execution data.

Format: projects/{project}/locations/{location}/keyRings/{keyRing}/cryptoKeys/{cryptoKey}</rdfs:comment>
    <rdfs:domain rdf:resource="http://example.org/onto/class/google_workflows_workflow"/>
    <rdfs:range rdf:resource="http://www.w3.org/2001/XMLSchema#string"/>
  </owl:DatatypeProperty>
  <owl:DatatypeProperty rdf:about="http://example.org/onto/prop/google_workflows_workflow_deletion_protection">
    <rdfs:label>deletion_protection</rdfs:label>
    <rdfs:comment>Whether Terraform will be prevented from destroying the workflow. Defaults to true.
When a'terraform destroy' or 'terraform apply' would delete the workflow,
the command will fail if this field is not set to false in Terraform state.
When the field is set to true or unset in Terraform state, a 'terraform apply'
or 'terraform destroy' that would delete the workflow will fail.
When the field is set to false, deleting the workflow is allowed.</rdfs:comment>
    <rdfs:domain rdf:resource="http://example.org/onto/class/google_workflows_workflow"/>
    <rdfs:range rdf:resource="http://www.w3.org/2001/XMLSchema#string"/>
  </owl:DatatypeProperty>
  <owl:DatatypeProperty rdf:about="http://example.org/onto/prop/google_workflows_workflow_description">
    <rdfs:label>description</rdfs:label>
    <rdfs:comment>Description of the workflow provided by the user. Must be at most 1000 unicode characters long.</rdfs:comment>
    <rdfs:domain rdf:resource="http://example.org/onto/class/google_workflows_workflow"/>
    <rdfs:range rdf:resource="http://www.w3.org/2001/XMLSchema#string"/>
  </owl:DatatypeProperty>
  <owl:DatatypeProperty rdf:about="http://example.org/onto/prop/google_workflows_workflow_effective_labels">
    <rdfs:label>effective_labels</rdfs:label>
    <rdfs:comment>All of labels (key/value pairs) present on the resource in GCP, including the labels configured through Terraform, other clients and services.</rdfs:comment>
    <rdfs:domain rdf:resource="http://example.org/onto/class/google_workflows_workflow"/>
    <rdfs:range rdf:resource="http://www.w3.org/2001/XMLSchema#string"/>
  </owl:DatatypeProperty>
  <owl:DatatypeProperty rdf:about="http://example.org/onto/prop/google_workflows_workflow_execution_history_level">
    <rdfs:label>execution_history_level</rdfs:label>
    <rdfs:comment>Describes the level of execution history to be stored for this workflow. This configuration
determines how much information about workflow executions is preserved. If not specified,
defaults to EXECUTION_HISTORY_LEVEL_UNSPECIFIED. Possible values: ["EXECUTION_HISTORY_LEVEL_UNSPECIFIED", "EXECUTION_HISTORY_BASIC", "EXECUTION_HISTORY_DETAILED"]</rdfs:comment>
    <rdfs:domain rdf:resource="http://example.org/onto/class/google_workflows_workflow"/>
    <rdfs:range rdf:resource="http://www.w3.org/2001/XMLSchema#string"/>
  </owl:DatatypeProperty>
  <owl:DatatypeProperty rdf:about="http://example.org/onto/prop/google_workflows_workflow_id">
    <rdfs:label>id</rdfs:label>
    <rdfs:domain rdf:resource="http://example.org/onto/class/google_workflows_workflow"/>
    <rdfs:range rdf:resource="http://www.w3.org/2001/XMLSchema#string"/>
  </owl:DatatypeProperty>
  <owl:DatatypeProperty rdf:about="http://example.org/onto/prop/google_workflows_workflow_labels">
    <rdfs:label>labels</rdfs:label>
    <rdfs:comment>A set of key/value label pairs to assign to this Workflow.


**Note**: This field is non-authoritative, and will only manage the labels present in your configuration.
Please refer to the field 'effective_labels' for all of the labels present on the resource.</rdfs:comment>
    <rdfs:domain rdf:resource="http://example.org/onto/class/google_workflows_workflow"/>
    <rdfs:range rdf:resource="http://www.w3.org/2001/XMLSchema#string"/>
  </owl:DatatypeProperty>
  <owl:DatatypeProperty rdf:about="http://example.org/onto/prop/google_workflows_workflow_name">
    <rdfs:label>name</rdfs:label>
    <rdfs:comment>Name of the Workflow.</rdfs:comment>
    <rdfs:domain rdf:resource="http://example.org/onto/class/google_workflows_workflow"/>
    <rdfs:range rdf:resource="http://www.w3.org/2001/XMLSchema#string"/>
  </owl:DatatypeProperty>
  <owl:DatatypeProperty rdf:about="http://example.org/onto/prop/google_workflows_workflow_name_prefix">
    <rdfs:label>name_prefix</rdfs:label>
    <rdfs:domain rdf:resource="http://example.org/onto/class/google_workflows_workflow"/>
    <rdfs:range rdf:resource="http://www.w3.org/2001/XMLSchema#string"/>
  </owl:DatatypeProperty>
  <owl:DatatypeProperty rdf:about="http://example.org/onto/prop/google_workflows_workflow_project">
    <rdfs:label>project</rdfs:label>
    <rdfs:domain rdf:resource="http://example.org/onto/class/google_workflows_workflow"/>
    <rdfs:range rdf:resource="http://www.w3.org/2001/XMLSchema#string"/>
  </owl:DatatypeProperty>
  <owl:DatatypeProperty rdf:about="http://example.org/onto/prop/google_workflows_workflow_region">
    <rdfs:label>region</rdfs:label>
    <rdfs:comment>The region of the workflow.</rdfs:comment>
    <rdfs:domain rdf:resource="http://example.org/onto/class/google_workflows_workflow"/>
    <rdfs:range rdf:resource="http://www.w3.org/2001/XMLSchema#string"/>
  </owl:DatatypeProperty>
  <owl:DatatypeProperty rdf:about="http://example.org/onto/prop/google_workflows_workflow_revision_id">
    <rdfs:label>revision_id</rdfs:label>
    <rdfs:comment>The revision of the workflow. A new one is generated if the service account or source contents is changed.</rdfs:comment>
    <rdfs:domain rdf:resource="http://example.org/onto/class/google_workflows_workflow"/>
    <rdfs:range rdf:resource="http://www.w3.org/2001/XMLSchema#string"/>
  </owl:DatatypeProperty>
  <owl:DatatypeProperty rdf:about="http://example.org/onto/prop/google_workflows_workflow_service_account">
    <rdfs:label>service_account</rdfs:label>
    <rdfs:comment>Name of the service account associated with the latest workflow version. This service
account represents the identity of the workflow and determines what permissions the workflow has.
Format: projects/{project}/serviceAccounts/{account} or {account}.
Using - as a wildcard for the {project} or not providing one at all will infer the project from the account.
The {account} value can be the email address or the unique_id of the service account.
If not provided, workflow will use the project's default service account.
Modifying this field for an existing workflow results in a new workflow revision.</rdfs:comment>
    <rdfs:domain rdf:resource="http://example.org/onto/class/google_workflows_workflow"/>
    <rdfs:range rdf:resource="http://www.w3.org/2001/XMLSchema#string"/>
  </owl:DatatypeProperty>
  <owl:DatatypeProperty rdf:about="http://example.org/onto/prop/google_workflows_workflow_source_contents">
    <rdfs:label>source_contents</rdfs:label>
    <rdfs:comment>Workflow code to be executed. The size limit is 128KB.</rdfs:comment>
    <rdfs:domain rdf:resource="http://example.org/onto/class/google_workflows_workflow"/>
    <rdfs:range rdf:resource="http://www.w3.org/2001/XMLSchema#string"/>
  </owl:DatatypeProperty>
  <owl:DatatypeProperty rdf:about="http://example.org/onto/prop/google_workflows_workflow_state">
    <rdfs:label>state</rdfs:label>
    <rdfs:comment>State of the workflow deployment.</rdfs:comment>
    <rdfs:domain rdf:resource="http://example.org/onto/class/google_workflows_workflow"/>
    <rdfs:range rdf:resource="http://www.w3.org/2001/XMLSchema#string"/>
  </owl:DatatypeProperty>
  <owl:DatatypeProperty rdf:about="http://example.org/onto/prop/google_workflows_workflow_tags">
    <rdfs:label>tags</rdfs:label>
    <rdfs:comment>A map of resource manager tags. Resource manager tag keys and values have the same definition
as resource manager tags. Keys must be in the format tagKeys/{tag_key_id}, and values are in
the format tagValues/456. The field is ignored (both PUT & PATCH) when empty.</rdfs:comment>
    <rdfs:domain rdf:resource="http://example.org/onto/class/google_workflows_workflow"/>
    <rdfs:range rdf:resource="http://www.w3.org/2001/XMLSchema#string"/>
  </owl:DatatypeProperty>
  <owl:DatatypeProperty rdf:about="http://example.org/onto/prop/google_workflows_workflow_terraform_labels">
    <rdfs:label>terraform_labels</rdfs:label>
    <rdfs:comment>The combination of labels configured directly on the resource
 and default labels configured on the provider.</rdfs:comment>
    <rdfs:domain rdf:resource="http://example.org/onto/class/google_workflows_workflow"/>
    <rdfs:range rdf:resource="http://www.w3.org/2001/XMLSchema#string"/>
  </owl:DatatypeProperty>
  <owl:DatatypeProperty rdf:about="http://example.org/onto/prop/google_workflows_workflow_update_time">
    <rdfs:label>update_time</rdfs:label>
    <rdfs:comment>The timestamp of when the workflow was last updated in RFC3339 UTC "Zulu" format, with nanosecond resolution and up to nine fractional digits.</rdfs:comment>
    <rdfs:domain rdf:resource="http://example.org/onto/class/google_workflows_workflow"/>
    <rdfs:range rdf:resource="http://www.w3.org/2001/XMLSchema#string"/>
  </owl:DatatypeProperty>
  <owl:DatatypeProperty rdf:about="http://example.org/onto/prop/google_workflows_workflow_user_env_vars">
    <rdfs:label>user_env_vars</rdfs:label>
    <rdfs:comment>User-defined environment variables associated with this workflow revision. This map has a maximum length of 20. Each string can take up to 4KiB. Keys cannot be empty strings and cannot start with "GOOGLE" or "WORKFLOWS".</rdfs:comment>
    <rdfs:domain rdf:resource="http://example.org/onto/class/google_workflows_workflow"/>
    <rdfs:range rdf:resource="http://www.w3.org/2001/XMLSchema#string"/>
  </owl:DatatypeProperty>
  <owl:DatatypeProperty rdf:about="http://example.org/onto/prop/google_workflows_workflow_create">
    <rdfs:label>create</rdfs:label>
    <rdfs:domain rdf:resource="http://example.org/onto/class/google_workflows_workflow"/>
    <rdfs:range rdf:resource="http://www.w3.org/2001/XMLSchema#string"/>
  </owl:DatatypeProperty>
  <owl:DatatypeProperty rdf:about="http://example.org/onto/prop/google_workflows_workflow_delete">
    <rdfs:label>delete</rdfs:label>
    <rdfs:domain rdf:resource="http://example.org/onto/class/google_workflows_workflow"/>
    <rdfs:range rdf:resource="http://www.w3.org/2001/XMLSchema#string"/>
  </owl:DatatypeProperty>
  <owl:DatatypeProperty rdf:about="http://example.org/onto/prop/google_workflows_workflow_update">
    <rdfs:label>update</rdfs:label>
    <rdfs:domain rdf:resource="http://example.org/onto/class/google_workflows_workflow"/>
    <rdfs:range rdf:resource="http://www.w3.org/2001/XMLSchema#string"/>
  </owl:DatatypeProperty>
</rdf:RDF>
