<?xml version="1.0" encoding="UTF-8"?>
<rdf:RDF
  xmlns:rdf="http://www.w3.org/1999/02/22-rdf-syntax-ns#"
  xmlns:rdfs="http://www.w3.org/2000/01/rdf-schema#"
  xmlns:owl="http://www.w3.org/2002/07/owl#"
  xmlns:xsd="http://www.w3.org/2001/XMLSchema#"
  xml:base="http://example.org/onto/">
  <owl:Class rdf:about="http://example.org/onto/class/google_app_engine_domain_mapping">
    <rdfs:label>google_app_engine_domain_mapping</rdfs:label>
    <rdfs:comment>#
#     ***     AUTO GENERATED CODE    ***    Type: MMv1     ***
#
# ----------------------------------------------------------------------------
#
#     This code is generated by Magic Modules using the following:
#
#     Configuration: https:#github.com/GoogleCloudPlatform/magic-modules/tree/main/mmv1/products/appengine/DomainMapping.yaml
#     Template:      https:#github.com/GoogleCloudPlatform/magic-modules/tree/main/mmv1/templates/terraform/resource.html.markdown.tmpl
#
#     DO NOT EDIT this file directly. Any changes made to this file will be
#     overwritten during the next generation cycle.
#
# ----------------------------------------------------------------------------
subcategory: "App Engine"
description: |-
  A domain serving an App Engine application.
---</rdfs:comment>
  </owl:Class>
  <owl:DatatypeProperty rdf:about="http://example.org/onto/prop/google_app_engine_domain_mapping_domain_name">
    <rdfs:label>domain_name</rdfs:label>
    <rdfs:comment>Relative name of the domain serving the application. Example: example.com.</rdfs:comment>
    <rdfs:domain rdf:resource="http://example.org/onto/class/google_app_engine_domain_mapping"/>
    <rdfs:range rdf:resource="http://www.w3.org/2001/XMLSchema#string"/>
  </owl:DatatypeProperty>
  <owl:DatatypeProperty rdf:about="http://example.org/onto/prop/google_app_engine_domain_mapping_id">
    <rdfs:label>id</rdfs:label>
    <rdfs:domain rdf:resource="http://example.org/onto/class/google_app_engine_domain_mapping"/>
    <rdfs:range rdf:resource="http://www.w3.org/2001/XMLSchema#string"/>
  </owl:DatatypeProperty>
  <owl:DatatypeProperty rdf:about="http://example.org/onto/prop/google_app_engine_domain_mapping_name">
    <rdfs:label>name</rdfs:label>
    <rdfs:comment>Full path to the DomainMapping resource in the API. Example: apps/myapp/domainMapping/example.com.</rdfs:comment>
    <rdfs:domain rdf:resource="http://example.org/onto/class/google_app_engine_domain_mapping"/>
    <rdfs:range rdf:resource="http://www.w3.org/2001/XMLSchema#string"/>
  </owl:DatatypeProperty>
  <owl:DatatypeProperty rdf:about="http://example.org/onto/prop/google_app_engine_domain_mapping_override_strategy">
    <rdfs:label>override_strategy</rdfs:label>
    <rdfs:comment>Whether the domain creation should override any existing mappings for this domain.
By default, overrides are rejected. Default value: "STRICT" Possible values: ["STRICT", "OVERRIDE"]</rdfs:comment>
    <rdfs:domain rdf:resource="http://example.org/onto/class/google_app_engine_domain_mapping"/>
    <rdfs:range rdf:resource="http://www.w3.org/2001/XMLSchema#string"/>
  </owl:DatatypeProperty>
  <owl:DatatypeProperty rdf:about="http://example.org/onto/prop/google_app_engine_domain_mapping_project">
    <rdfs:label>project</rdfs:label>
    <rdfs:domain rdf:resource="http://example.org/onto/class/google_app_engine_domain_mapping"/>
    <rdfs:range rdf:resource="http://www.w3.org/2001/XMLSchema#string"/>
  </owl:DatatypeProperty>
  <owl:DatatypeProperty rdf:about="http://example.org/onto/prop/google_app_engine_domain_mapping_resource_records">
    <rdfs:label>resource_records</rdfs:label>
    <rdfs:comment>The resource records required to configure this domain mapping. These records must be added to the domain's DNS
configuration in order to serve the application via this domain mapping.</rdfs:comment>
    <rdfs:domain rdf:resource="http://example.org/onto/class/google_app_engine_domain_mapping"/>
    <rdfs:range rdf:resource="http://www.w3.org/2001/XMLSchema#string"/>
  </owl:DatatypeProperty>
  <owl:DatatypeProperty rdf:about="http://example.org/onto/prop/google_app_engine_domain_mapping_certificate_id">
    <rdfs:label>certificate_id</rdfs:label>
    <rdfs:comment>ID of the AuthorizedCertificate resource configuring SSL for the application. Clearing this field will
remove SSL support.
By default, a managed certificate is automatically created for every domain mapping. To omit SSL support
or to configure SSL manually, specify 'SslManagementType.MANUAL' on a 'CREATE' or 'UPDATE' request. You must be
authorized to administer the 'AuthorizedCertificate' resource to manually map it to a DomainMapping resource.
Example: 12345.</rdfs:comment>
    <rdfs:domain rdf:resource="http://example.org/onto/class/google_app_engine_domain_mapping"/>
    <rdfs:range rdf:resource="http://www.w3.org/2001/XMLSchema#string"/>
  </owl:DatatypeProperty>
  <owl:DatatypeProperty rdf:about="http://example.org/onto/prop/google_app_engine_domain_mapping_pending_managed_certificate_id">
    <rdfs:label>pending_managed_certificate_id</rdfs:label>
    <rdfs:comment>ID of the managed 'AuthorizedCertificate' resource currently being provisioned, if applicable. Until the new
managed certificate has been successfully provisioned, the previous SSL state will be preserved. Once the
provisioning process completes, the 'certificateId' field will reflect the new managed certificate and this
field will be left empty. To remove SSL support while there is still a pending managed certificate, clear the
'certificateId' field with an update request.</rdfs:comment>
    <rdfs:domain rdf:resource="http://example.org/onto/class/google_app_engine_domain_mapping"/>
    <rdfs:range rdf:resource="http://www.w3.org/2001/XMLSchema#string"/>
  </owl:DatatypeProperty>
  <owl:DatatypeProperty rdf:about="http://example.org/onto/prop/google_app_engine_domain_mapping_ssl_management_type">
    <rdfs:label>ssl_management_type</rdfs:label>
    <rdfs:comment>SSL management type for this domain. If 'AUTOMATIC', a managed certificate is automatically provisioned.
If 'MANUAL', 'certificateId' must be manually specified in order to configure SSL for this domain. Possible values: ["AUTOMATIC", "MANUAL"]</rdfs:comment>
    <rdfs:domain rdf:resource="http://example.org/onto/class/google_app_engine_domain_mapping"/>
    <rdfs:range rdf:resource="http://www.w3.org/2001/XMLSchema#string"/>
  </owl:DatatypeProperty>
  <owl:DatatypeProperty rdf:about="http://example.org/onto/prop/google_app_engine_domain_mapping_create">
    <rdfs:label>create</rdfs:label>
    <rdfs:domain rdf:resource="http://example.org/onto/class/google_app_engine_domain_mapping"/>
    <rdfs:range rdf:resource="http://www.w3.org/2001/XMLSchema#string"/>
  </owl:DatatypeProperty>
  <owl:DatatypeProperty rdf:about="http://example.org/onto/prop/google_app_engine_domain_mapping_delete">
    <rdfs:label>delete</rdfs:label>
    <rdfs:domain rdf:resource="http://example.org/onto/class/google_app_engine_domain_mapping"/>
    <rdfs:range rdf:resource="http://www.w3.org/2001/XMLSchema#string"/>
  </owl:DatatypeProperty>
  <owl:DatatypeProperty rdf:about="http://example.org/onto/prop/google_app_engine_domain_mapping_update">
    <rdfs:label>update</rdfs:label>
    <rdfs:domain rdf:resource="http://example.org/onto/class/google_app_engine_domain_mapping"/>
    <rdfs:range rdf:resource="http://www.w3.org/2001/XMLSchema#string"/>
  </owl:DatatypeProperty>
</rdf:RDF>
