<?xml version="1.0" encoding="UTF-8"?>
<rdf:RDF
  xmlns:rdf="http://www.w3.org/1999/02/22-rdf-syntax-ns#"
  xmlns:rdfs="http://www.w3.org/2000/01/rdf-schema#"
  xmlns:owl="http://www.w3.org/2002/07/owl#"
  xmlns:xsd="http://www.w3.org/2001/XMLSchema#"
  xml:base="http://example.org/onto/">
  <owl:Class rdf:about="http://example.org/onto/class/google_network_management_vpc_flow_logs_config">
    <rdfs:label>google_network_management_vpc_flow_logs_config</rdfs:label>
    <rdfs:comment>#
#     ***     AUTO GENERATED CODE    ***    Type: MMv1     ***
#
# ----------------------------------------------------------------------------
#
#     This code is generated by Magic Modules using the following:
#
#     Configuration: https:#github.com/GoogleCloudPlatform/magic-modules/tree/main/mmv1/products/networkmanagement/VpcFlowLogsConfig.yaml
#     Template:      https:#github.com/GoogleCloudPlatform/magic-modules/tree/main/mmv1/templates/terraform/resource.html.markdown.tmpl
#
#     DO NOT EDIT this file directly. Any changes made to this file will be
#     overwritten during the next generation cycle.
#
# ----------------------------------------------------------------------------
subcategory: "Network Management"
description: |-
  VPC Flow Logs Config is a resource that lets you configure Flow Logs for Networks, Subnets, Interconnect attachments or VPN Tunnels.
---</rdfs:comment>
  </owl:Class>
  <owl:DatatypeProperty rdf:about="http://example.org/onto/prop/google_network_management_vpc_flow_logs_config_aggregation_interval">
    <rdfs:label>aggregation_interval</rdfs:label>
    <rdfs:comment>Optional. The aggregation interval for the logs. Default value is
INTERVAL_5_SEC.   Possible values:  AGGREGATION_INTERVAL_UNSPECIFIED INTERVAL_5_SEC INTERVAL_30_SEC INTERVAL_1_MIN INTERVAL_5_MIN INTERVAL_10_MIN INTERVAL_15_MIN</rdfs:comment>
    <rdfs:domain rdf:resource="http://example.org/onto/class/google_network_management_vpc_flow_logs_config"/>
    <rdfs:range rdf:resource="http://www.w3.org/2001/XMLSchema#string"/>
  </owl:DatatypeProperty>
  <owl:DatatypeProperty rdf:about="http://example.org/onto/prop/google_network_management_vpc_flow_logs_config_create_time">
    <rdfs:label>create_time</rdfs:label>
    <rdfs:comment>Output only. The time the config was created.</rdfs:comment>
    <rdfs:domain rdf:resource="http://example.org/onto/class/google_network_management_vpc_flow_logs_config"/>
    <rdfs:range rdf:resource="http://www.w3.org/2001/XMLSchema#string"/>
  </owl:DatatypeProperty>
  <owl:DatatypeProperty rdf:about="http://example.org/onto/prop/google_network_management_vpc_flow_logs_config_description">
    <rdfs:label>description</rdfs:label>
    <rdfs:comment>Optional. The user-supplied description of the VPC Flow Logs configuration. Maximum
of 512 characters.</rdfs:comment>
    <rdfs:domain rdf:resource="http://example.org/onto/class/google_network_management_vpc_flow_logs_config"/>
    <rdfs:range rdf:resource="http://www.w3.org/2001/XMLSchema#string"/>
  </owl:DatatypeProperty>
  <owl:DatatypeProperty rdf:about="http://example.org/onto/prop/google_network_management_vpc_flow_logs_config_effective_labels">
    <rdfs:label>effective_labels</rdfs:label>
    <rdfs:comment>All of labels (key/value pairs) present on the resource in GCP, including the labels configured through Terraform, other clients and services.</rdfs:comment>
    <rdfs:domain rdf:resource="http://example.org/onto/class/google_network_management_vpc_flow_logs_config"/>
    <rdfs:range rdf:resource="http://www.w3.org/2001/XMLSchema#string"/>
  </owl:DatatypeProperty>
  <owl:DatatypeProperty rdf:about="http://example.org/onto/prop/google_network_management_vpc_flow_logs_config_filter_expr">
    <rdfs:label>filter_expr</rdfs:label>
    <rdfs:comment>Optional. Export filter used to define which VPC Flow Logs should be logged.</rdfs:comment>
    <rdfs:domain rdf:resource="http://example.org/onto/class/google_network_management_vpc_flow_logs_config"/>
    <rdfs:range rdf:resource="http://www.w3.org/2001/XMLSchema#string"/>
  </owl:DatatypeProperty>
  <owl:DatatypeProperty rdf:about="http://example.org/onto/prop/google_network_management_vpc_flow_logs_config_flow_sampling">
    <rdfs:label>flow_sampling</rdfs:label>
    <rdfs:comment>Optional. The value of the field must be in (0, 1]. The sampling rate
of VPC Flow Logs where 1.0 means all collected logs are reported. Setting the
sampling rate to 0.0 is not allowed. If you want to disable VPC Flow Logs, use
the state field instead. Default value is 1.0.</rdfs:comment>
    <rdfs:domain rdf:resource="http://example.org/onto/class/google_network_management_vpc_flow_logs_config"/>
    <rdfs:range rdf:resource="http://www.w3.org/2001/XMLSchema#string"/>
  </owl:DatatypeProperty>
  <owl:DatatypeProperty rdf:about="http://example.org/onto/prop/google_network_management_vpc_flow_logs_config_id">
    <rdfs:label>id</rdfs:label>
    <rdfs:domain rdf:resource="http://example.org/onto/class/google_network_management_vpc_flow_logs_config"/>
    <rdfs:range rdf:resource="http://www.w3.org/2001/XMLSchema#string"/>
  </owl:DatatypeProperty>
  <owl:DatatypeProperty rdf:about="http://example.org/onto/prop/google_network_management_vpc_flow_logs_config_interconnect_attachment">
    <rdfs:label>interconnect_attachment</rdfs:label>
    <rdfs:comment>Traffic will be logged from the Interconnect Attachment. Format: projects/{project_id}/regions/{region}/interconnectAttachments/{name}</rdfs:comment>
    <rdfs:domain rdf:resource="http://example.org/onto/class/google_network_management_vpc_flow_logs_config"/>
    <rdfs:range rdf:resource="http://www.w3.org/2001/XMLSchema#string"/>
  </owl:DatatypeProperty>
  <owl:DatatypeProperty rdf:about="http://example.org/onto/prop/google_network_management_vpc_flow_logs_config_labels">
    <rdfs:label>labels</rdfs:label>
    <rdfs:comment>Optional. Resource labels to represent user-provided metadata.


**Note**: This field is non-authoritative, and will only manage the labels present in your configuration.
Please refer to the field 'effective_labels' for all of the labels present on the resource.</rdfs:comment>
    <rdfs:domain rdf:resource="http://example.org/onto/class/google_network_management_vpc_flow_logs_config"/>
    <rdfs:range rdf:resource="http://www.w3.org/2001/XMLSchema#string"/>
  </owl:DatatypeProperty>
  <owl:DatatypeProperty rdf:about="http://example.org/onto/prop/google_network_management_vpc_flow_logs_config_location">
    <rdfs:label>location</rdfs:label>
    <rdfs:comment>Resource ID segment making up resource 'name'. It identifies the resource
within its parent collection as described in https://google.aip.dev/122. See documentation
for resource type 'networkmanagement.googleapis.com/VpcFlowLogsConfig'.</rdfs:comment>
    <rdfs:domain rdf:resource="http://example.org/onto/class/google_network_management_vpc_flow_logs_config"/>
    <rdfs:range rdf:resource="http://www.w3.org/2001/XMLSchema#string"/>
  </owl:DatatypeProperty>
  <owl:DatatypeProperty rdf:about="http://example.org/onto/prop/google_network_management_vpc_flow_logs_config_metadata">
    <rdfs:label>metadata</rdfs:label>
    <rdfs:comment>Optional. Configures whether all, none or a subset of metadata fields
should be added to the reported VPC flow logs. Default value is INCLUDE_ALL_METADATA.
  Possible values:  METADATA_UNSPECIFIED INCLUDE_ALL_METADATA EXCLUDE_ALL_METADATA CUSTOM_METADATA</rdfs:comment>
    <rdfs:domain rdf:resource="http://example.org/onto/class/google_network_management_vpc_flow_logs_config"/>
    <rdfs:range rdf:resource="http://www.w3.org/2001/XMLSchema#string"/>
  </owl:DatatypeProperty>
  <owl:DatatypeProperty rdf:about="http://example.org/onto/prop/google_network_management_vpc_flow_logs_config_metadata_fields">
    <rdfs:label>metadata_fields</rdfs:label>
    <rdfs:comment>Optional. Custom metadata fields to include in the reported VPC flow
logs. Can only be specified if \"metadata\" was set to CUSTOM_METADATA.</rdfs:comment>
    <rdfs:domain rdf:resource="http://example.org/onto/class/google_network_management_vpc_flow_logs_config"/>
    <rdfs:range rdf:resource="http://www.w3.org/2001/XMLSchema#string"/>
  </owl:DatatypeProperty>
  <owl:DatatypeProperty rdf:about="http://example.org/onto/prop/google_network_management_vpc_flow_logs_config_name">
    <rdfs:label>name</rdfs:label>
    <rdfs:comment>Identifier. Unique name of the configuration using the form:     'projects/{project_id}/locations/global/vpcFlowLogsConfigs/{vpc_flow_logs_config_id}'</rdfs:comment>
    <rdfs:domain rdf:resource="http://example.org/onto/class/google_network_management_vpc_flow_logs_config"/>
    <rdfs:range rdf:resource="http://www.w3.org/2001/XMLSchema#string"/>
  </owl:DatatypeProperty>
  <owl:DatatypeProperty rdf:about="http://example.org/onto/prop/google_network_management_vpc_flow_logs_config_project">
    <rdfs:label>project</rdfs:label>
    <rdfs:domain rdf:resource="http://example.org/onto/class/google_network_management_vpc_flow_logs_config"/>
    <rdfs:range rdf:resource="http://www.w3.org/2001/XMLSchema#string"/>
  </owl:DatatypeProperty>
  <owl:DatatypeProperty rdf:about="http://example.org/onto/prop/google_network_management_vpc_flow_logs_config_state">
    <rdfs:label>state</rdfs:label>
    <rdfs:comment>Optional. The state of the VPC Flow Log configuration. Default value
is ENABLED. When creating a new configuration, it must be enabled.
Possible values: STATE_UNSPECIFIED ENABLED DISABLED</rdfs:comment>
    <rdfs:domain rdf:resource="http://example.org/onto/class/google_network_management_vpc_flow_logs_config"/>
    <rdfs:range rdf:resource="http://www.w3.org/2001/XMLSchema#string"/>
  </owl:DatatypeProperty>
  <owl:DatatypeProperty rdf:about="http://example.org/onto/prop/google_network_management_vpc_flow_logs_config_target_resource_state">
    <rdfs:label>target_resource_state</rdfs:label>
    <rdfs:comment>Describes the state of the configured target resource for diagnostic
purposes.
Possible values:
TARGET_RESOURCE_STATE_UNSPECIFIED
TARGET_RESOURCE_EXISTS
TARGET_RESOURCE_DOES_NOT_EXIST</rdfs:comment>
    <rdfs:domain rdf:resource="http://example.org/onto/class/google_network_management_vpc_flow_logs_config"/>
    <rdfs:range rdf:resource="http://www.w3.org/2001/XMLSchema#string"/>
  </owl:DatatypeProperty>
  <owl:DatatypeProperty rdf:about="http://example.org/onto/prop/google_network_management_vpc_flow_logs_config_terraform_labels">
    <rdfs:label>terraform_labels</rdfs:label>
    <rdfs:comment>The combination of labels configured directly on the resource
 and default labels configured on the provider.</rdfs:comment>
    <rdfs:domain rdf:resource="http://example.org/onto/class/google_network_management_vpc_flow_logs_config"/>
    <rdfs:range rdf:resource="http://www.w3.org/2001/XMLSchema#string"/>
  </owl:DatatypeProperty>
  <owl:DatatypeProperty rdf:about="http://example.org/onto/prop/google_network_management_vpc_flow_logs_config_update_time">
    <rdfs:label>update_time</rdfs:label>
    <rdfs:comment>Output only. The time the config was updated.</rdfs:comment>
    <rdfs:domain rdf:resource="http://example.org/onto/class/google_network_management_vpc_flow_logs_config"/>
    <rdfs:range rdf:resource="http://www.w3.org/2001/XMLSchema#string"/>
  </owl:DatatypeProperty>
  <owl:DatatypeProperty rdf:about="http://example.org/onto/prop/google_network_management_vpc_flow_logs_config_vpc_flow_logs_config_id">
    <rdfs:label>vpc_flow_logs_config_id</rdfs:label>
    <rdfs:comment>Required. ID of the 'VpcFlowLogsConfig'.</rdfs:comment>
    <rdfs:domain rdf:resource="http://example.org/onto/class/google_network_management_vpc_flow_logs_config"/>
    <rdfs:range rdf:resource="http://www.w3.org/2001/XMLSchema#string"/>
  </owl:DatatypeProperty>
  <owl:DatatypeProperty rdf:about="http://example.org/onto/prop/google_network_management_vpc_flow_logs_config_vpn_tunnel">
    <rdfs:label>vpn_tunnel</rdfs:label>
    <rdfs:comment>Traffic will be logged from the VPN Tunnel. Format: projects/{project_id}/regions/{region}/vpnTunnels/{name}</rdfs:comment>
    <rdfs:domain rdf:resource="http://example.org/onto/class/google_network_management_vpc_flow_logs_config"/>
    <rdfs:range rdf:resource="http://www.w3.org/2001/XMLSchema#string"/>
  </owl:DatatypeProperty>
  <owl:DatatypeProperty rdf:about="http://example.org/onto/prop/google_network_management_vpc_flow_logs_config_create">
    <rdfs:label>create</rdfs:label>
    <rdfs:domain rdf:resource="http://example.org/onto/class/google_network_management_vpc_flow_logs_config"/>
    <rdfs:range rdf:resource="http://www.w3.org/2001/XMLSchema#string"/>
  </owl:DatatypeProperty>
  <owl:DatatypeProperty rdf:about="http://example.org/onto/prop/google_network_management_vpc_flow_logs_config_delete">
    <rdfs:label>delete</rdfs:label>
    <rdfs:domain rdf:resource="http://example.org/onto/class/google_network_management_vpc_flow_logs_config"/>
    <rdfs:range rdf:resource="http://www.w3.org/2001/XMLSchema#string"/>
  </owl:DatatypeProperty>
  <owl:DatatypeProperty rdf:about="http://example.org/onto/prop/google_network_management_vpc_flow_logs_config_update">
    <rdfs:label>update</rdfs:label>
    <rdfs:domain rdf:resource="http://example.org/onto/class/google_network_management_vpc_flow_logs_config"/>
    <rdfs:range rdf:resource="http://www.w3.org/2001/XMLSchema#string"/>
  </owl:DatatypeProperty>
</rdf:RDF>
