<?xml version="1.0" encoding="UTF-8"?>
<rdf:RDF
  xmlns:rdf="http://www.w3.org/1999/02/22-rdf-syntax-ns#"
  xmlns:rdfs="http://www.w3.org/2000/01/rdf-schema#"
  xmlns:owl="http://www.w3.org/2002/07/owl#"
  xmlns:xsd="http://www.w3.org/2001/XMLSchema#"
  xml:base="http://example.org/onto/">
  <owl:Class rdf:about="http://example.org/onto/class/google_compute_https_health_check">
    <rdfs:label>google_compute_https_health_check</rdfs:label>
    <rdfs:comment>#
#     ***     AUTO GENERATED CODE    ***    Type: MMv1     ***
#
# ----------------------------------------------------------------------------
#
#     This code is generated by Magic Modules using the following:
#
#     Configuration: https:#github.com/GoogleCloudPlatform/magic-modules/tree/main/mmv1/products/compute/HttpsHealthCheck.yaml
#     Template:      https:#github.com/GoogleCloudPlatform/magic-modules/tree/main/mmv1/templates/terraform/resource.html.markdown.tmpl
#
#     DO NOT EDIT this file directly. Any changes made to this file will be
#     overwritten during the next generation cycle.
#
# ----------------------------------------------------------------------------
subcategory: "Compute Engine"
description: |-
  An HttpsHealthCheck resource.
---</rdfs:comment>
  </owl:Class>
  <owl:DatatypeProperty rdf:about="http://example.org/onto/prop/google_compute_https_health_check_check_interval_sec">
    <rdfs:label>check_interval_sec</rdfs:label>
    <rdfs:comment>How often (in seconds) to send a health check. The default value is 5
seconds.</rdfs:comment>
    <rdfs:domain rdf:resource="http://example.org/onto/class/google_compute_https_health_check"/>
    <rdfs:range rdf:resource="http://www.w3.org/2001/XMLSchema#string"/>
  </owl:DatatypeProperty>
  <owl:DatatypeProperty rdf:about="http://example.org/onto/prop/google_compute_https_health_check_creation_timestamp">
    <rdfs:label>creation_timestamp</rdfs:label>
    <rdfs:comment>Creation timestamp in RFC3339 text format.</rdfs:comment>
    <rdfs:domain rdf:resource="http://example.org/onto/class/google_compute_https_health_check"/>
    <rdfs:range rdf:resource="http://www.w3.org/2001/XMLSchema#string"/>
  </owl:DatatypeProperty>
  <owl:DatatypeProperty rdf:about="http://example.org/onto/prop/google_compute_https_health_check_description">
    <rdfs:label>description</rdfs:label>
    <rdfs:comment>An optional description of this resource. Provide this property when
you create the resource.</rdfs:comment>
    <rdfs:domain rdf:resource="http://example.org/onto/class/google_compute_https_health_check"/>
    <rdfs:range rdf:resource="http://www.w3.org/2001/XMLSchema#string"/>
  </owl:DatatypeProperty>
  <owl:DatatypeProperty rdf:about="http://example.org/onto/prop/google_compute_https_health_check_healthy_threshold">
    <rdfs:label>healthy_threshold</rdfs:label>
    <rdfs:comment>A so-far unhealthy instance will be marked healthy after this many
consecutive successes. The default value is 2.</rdfs:comment>
    <rdfs:domain rdf:resource="http://example.org/onto/class/google_compute_https_health_check"/>
    <rdfs:range rdf:resource="http://www.w3.org/2001/XMLSchema#string"/>
  </owl:DatatypeProperty>
  <owl:DatatypeProperty rdf:about="http://example.org/onto/prop/google_compute_https_health_check_host">
    <rdfs:label>host</rdfs:label>
    <rdfs:comment>The value of the host header in the HTTPS health check request. If
left empty (default value), the public IP on behalf of which this
health check is performed will be used.</rdfs:comment>
    <rdfs:domain rdf:resource="http://example.org/onto/class/google_compute_https_health_check"/>
    <rdfs:range rdf:resource="http://www.w3.org/2001/XMLSchema#string"/>
  </owl:DatatypeProperty>
  <owl:DatatypeProperty rdf:about="http://example.org/onto/prop/google_compute_https_health_check_id">
    <rdfs:label>id</rdfs:label>
    <rdfs:domain rdf:resource="http://example.org/onto/class/google_compute_https_health_check"/>
    <rdfs:range rdf:resource="http://www.w3.org/2001/XMLSchema#string"/>
  </owl:DatatypeProperty>
  <owl:DatatypeProperty rdf:about="http://example.org/onto/prop/google_compute_https_health_check_name">
    <rdfs:label>name</rdfs:label>
    <rdfs:comment>Name of the resource. Provided by the client when the resource is
created. The name must be 1-63 characters long, and comply with
RFC1035.  Specifically, the name must be 1-63 characters long and
match the regular expression '[a-z]([-a-z0-9]*[a-z0-9])?' which means
the first character must be a lowercase letter, and all following
characters must be a dash, lowercase letter, or digit, except the
last character, which cannot be a dash.</rdfs:comment>
    <rdfs:domain rdf:resource="http://example.org/onto/class/google_compute_https_health_check"/>
    <rdfs:range rdf:resource="http://www.w3.org/2001/XMLSchema#string"/>
  </owl:DatatypeProperty>
  <owl:DatatypeProperty rdf:about="http://example.org/onto/prop/google_compute_https_health_check_port">
    <rdfs:label>port</rdfs:label>
    <rdfs:comment>The TCP port number for the HTTPS health check request.
The default value is 443.</rdfs:comment>
    <rdfs:domain rdf:resource="http://example.org/onto/class/google_compute_https_health_check"/>
    <rdfs:range rdf:resource="http://www.w3.org/2001/XMLSchema#string"/>
  </owl:DatatypeProperty>
  <owl:DatatypeProperty rdf:about="http://example.org/onto/prop/google_compute_https_health_check_project">
    <rdfs:label>project</rdfs:label>
    <rdfs:domain rdf:resource="http://example.org/onto/class/google_compute_https_health_check"/>
    <rdfs:range rdf:resource="http://www.w3.org/2001/XMLSchema#string"/>
  </owl:DatatypeProperty>
  <owl:DatatypeProperty rdf:about="http://example.org/onto/prop/google_compute_https_health_check_request_path">
    <rdfs:label>request_path</rdfs:label>
    <rdfs:comment>The request path of the HTTPS health check request.
The default value is /.</rdfs:comment>
    <rdfs:domain rdf:resource="http://example.org/onto/class/google_compute_https_health_check"/>
    <rdfs:range rdf:resource="http://www.w3.org/2001/XMLSchema#string"/>
  </owl:DatatypeProperty>
  <owl:DatatypeProperty rdf:about="http://example.org/onto/prop/google_compute_https_health_check_self_link">
    <rdfs:label>self_link</rdfs:label>
    <rdfs:domain rdf:resource="http://example.org/onto/class/google_compute_https_health_check"/>
    <rdfs:range rdf:resource="http://www.w3.org/2001/XMLSchema#string"/>
  </owl:DatatypeProperty>
  <owl:DatatypeProperty rdf:about="http://example.org/onto/prop/google_compute_https_health_check_timeout_sec">
    <rdfs:label>timeout_sec</rdfs:label>
    <rdfs:comment>How long (in seconds) to wait before claiming failure.
The default value is 5 seconds.  It is invalid for timeoutSec to have
greater value than checkIntervalSec.</rdfs:comment>
    <rdfs:domain rdf:resource="http://example.org/onto/class/google_compute_https_health_check"/>
    <rdfs:range rdf:resource="http://www.w3.org/2001/XMLSchema#string"/>
  </owl:DatatypeProperty>
  <owl:DatatypeProperty rdf:about="http://example.org/onto/prop/google_compute_https_health_check_unhealthy_threshold">
    <rdfs:label>unhealthy_threshold</rdfs:label>
    <rdfs:comment>A so-far healthy instance will be marked unhealthy after this many
consecutive failures. The default value is 2.</rdfs:comment>
    <rdfs:domain rdf:resource="http://example.org/onto/class/google_compute_https_health_check"/>
    <rdfs:range rdf:resource="http://www.w3.org/2001/XMLSchema#string"/>
  </owl:DatatypeProperty>
  <owl:DatatypeProperty rdf:about="http://example.org/onto/prop/google_compute_https_health_check_create">
    <rdfs:label>create</rdfs:label>
    <rdfs:domain rdf:resource="http://example.org/onto/class/google_compute_https_health_check"/>
    <rdfs:range rdf:resource="http://www.w3.org/2001/XMLSchema#string"/>
  </owl:DatatypeProperty>
  <owl:DatatypeProperty rdf:about="http://example.org/onto/prop/google_compute_https_health_check_delete">
    <rdfs:label>delete</rdfs:label>
    <rdfs:domain rdf:resource="http://example.org/onto/class/google_compute_https_health_check"/>
    <rdfs:range rdf:resource="http://www.w3.org/2001/XMLSchema#string"/>
  </owl:DatatypeProperty>
  <owl:DatatypeProperty rdf:about="http://example.org/onto/prop/google_compute_https_health_check_update">
    <rdfs:label>update</rdfs:label>
    <rdfs:domain rdf:resource="http://example.org/onto/class/google_compute_https_health_check"/>
    <rdfs:range rdf:resource="http://www.w3.org/2001/XMLSchema#string"/>
  </owl:DatatypeProperty>
</rdf:RDF>
