<?xml version="1.0" encoding="UTF-8"?>
<rdf:RDF
  xmlns:rdf="http://www.w3.org/1999/02/22-rdf-syntax-ns#"
  xmlns:rdfs="http://www.w3.org/2000/01/rdf-schema#"
  xmlns:owl="http://www.w3.org/2002/07/owl#"
  xmlns:xsd="http://www.w3.org/2001/XMLSchema#"
  xml:base="http://example.org/onto/">
  <owl:Class rdf:about="http://example.org/onto/class/google_data_loss_prevention_discovery_config">
    <rdfs:label>google_data_loss_prevention_discovery_config</rdfs:label>
    <rdfs:comment>#
#     ***     AUTO GENERATED CODE    ***    Type: MMv1     ***
#
# ----------------------------------------------------------------------------
#
#     This code is generated by Magic Modules using the following:
#
#     Configuration: https:#github.com/GoogleCloudPlatform/magic-modules/tree/main/mmv1/products/dlp/DiscoveryConfig.yaml
#     Template:      https:#github.com/GoogleCloudPlatform/magic-modules/tree/main/mmv1/templates/terraform/resource.html.markdown.tmpl
#
#     DO NOT EDIT this file directly. Any changes made to this file will be
#     overwritten during the next generation cycle.
#
# ----------------------------------------------------------------------------
subcategory: "Data Loss Prevention"
description: |-
  Configuration for discovery to scan resources for profile generation.
---</rdfs:comment>
  </owl:Class>
  <owl:DatatypeProperty rdf:about="http://example.org/onto/prop/google_data_loss_prevention_discovery_config_create_time">
    <rdfs:label>create_time</rdfs:label>
    <rdfs:comment>Output only. The creation timestamp of a DiscoveryConfig.</rdfs:comment>
    <rdfs:domain rdf:resource="http://example.org/onto/class/google_data_loss_prevention_discovery_config"/>
    <rdfs:range rdf:resource="http://www.w3.org/2001/XMLSchema#string"/>
  </owl:DatatypeProperty>
  <owl:DatatypeProperty rdf:about="http://example.org/onto/prop/google_data_loss_prevention_discovery_config_display_name">
    <rdfs:label>display_name</rdfs:label>
    <rdfs:comment>Display Name (max 1000 Chars)</rdfs:comment>
    <rdfs:domain rdf:resource="http://example.org/onto/class/google_data_loss_prevention_discovery_config"/>
    <rdfs:range rdf:resource="http://www.w3.org/2001/XMLSchema#string"/>
  </owl:DatatypeProperty>
  <owl:DatatypeProperty rdf:about="http://example.org/onto/prop/google_data_loss_prevention_discovery_config_errors">
    <rdfs:label>errors</rdfs:label>
    <rdfs:comment>Output only. A stream of errors encountered when the config was activated. Repeated errors may result in the config automatically being paused. Output only field. Will return the last 100 errors. Whenever the config is modified this list will be cleared.</rdfs:comment>
    <rdfs:domain rdf:resource="http://example.org/onto/class/google_data_loss_prevention_discovery_config"/>
    <rdfs:range rdf:resource="http://www.w3.org/2001/XMLSchema#string"/>
  </owl:DatatypeProperty>
  <owl:DatatypeProperty rdf:about="http://example.org/onto/prop/google_data_loss_prevention_discovery_config_id">
    <rdfs:label>id</rdfs:label>
    <rdfs:domain rdf:resource="http://example.org/onto/class/google_data_loss_prevention_discovery_config"/>
    <rdfs:range rdf:resource="http://www.w3.org/2001/XMLSchema#string"/>
  </owl:DatatypeProperty>
  <owl:DatatypeProperty rdf:about="http://example.org/onto/prop/google_data_loss_prevention_discovery_config_inspect_templates">
    <rdfs:label>inspect_templates</rdfs:label>
    <rdfs:comment>Detection logic for profile generation</rdfs:comment>
    <rdfs:domain rdf:resource="http://example.org/onto/class/google_data_loss_prevention_discovery_config"/>
    <rdfs:range rdf:resource="http://www.w3.org/2001/XMLSchema#string"/>
  </owl:DatatypeProperty>
  <owl:DatatypeProperty rdf:about="http://example.org/onto/prop/google_data_loss_prevention_discovery_config_last_run_time">
    <rdfs:label>last_run_time</rdfs:label>
    <rdfs:comment>Output only. The timestamp of the last time this config was executed</rdfs:comment>
    <rdfs:domain rdf:resource="http://example.org/onto/class/google_data_loss_prevention_discovery_config"/>
    <rdfs:range rdf:resource="http://www.w3.org/2001/XMLSchema#string"/>
  </owl:DatatypeProperty>
  <owl:DatatypeProperty rdf:about="http://example.org/onto/prop/google_data_loss_prevention_discovery_config_location">
    <rdfs:label>location</rdfs:label>
    <rdfs:comment>Location to create the discovery config in.</rdfs:comment>
    <rdfs:domain rdf:resource="http://example.org/onto/class/google_data_loss_prevention_discovery_config"/>
    <rdfs:range rdf:resource="http://www.w3.org/2001/XMLSchema#string"/>
  </owl:DatatypeProperty>
  <owl:DatatypeProperty rdf:about="http://example.org/onto/prop/google_data_loss_prevention_discovery_config_name">
    <rdfs:label>name</rdfs:label>
    <rdfs:comment>Unique resource name for the DiscoveryConfig, assigned by the service when the DiscoveryConfig is created.</rdfs:comment>
    <rdfs:domain rdf:resource="http://example.org/onto/class/google_data_loss_prevention_discovery_config"/>
    <rdfs:range rdf:resource="http://www.w3.org/2001/XMLSchema#string"/>
  </owl:DatatypeProperty>
  <owl:DatatypeProperty rdf:about="http://example.org/onto/prop/google_data_loss_prevention_discovery_config_parent">
    <rdfs:label>parent</rdfs:label>
    <rdfs:comment>The parent of the discovery config in any of the following formats:

* 'projects/{{project}}/locations/{{location}}'
* 'organizations/{{organization_id}}/locations/{{location}}'</rdfs:comment>
    <rdfs:domain rdf:resource="http://example.org/onto/class/google_data_loss_prevention_discovery_config"/>
    <rdfs:range rdf:resource="http://www.w3.org/2001/XMLSchema#string"/>
  </owl:DatatypeProperty>
  <owl:DatatypeProperty rdf:about="http://example.org/onto/prop/google_data_loss_prevention_discovery_config_status">
    <rdfs:label>status</rdfs:label>
    <rdfs:comment>Required. A status for this configuration Possible values: ["RUNNING", "PAUSED"]</rdfs:comment>
    <rdfs:domain rdf:resource="http://example.org/onto/class/google_data_loss_prevention_discovery_config"/>
    <rdfs:range rdf:resource="http://www.w3.org/2001/XMLSchema#string"/>
  </owl:DatatypeProperty>
  <owl:DatatypeProperty rdf:about="http://example.org/onto/prop/google_data_loss_prevention_discovery_config_update_time">
    <rdfs:label>update_time</rdfs:label>
    <rdfs:comment>Output only. The last update timestamp of a DiscoveryConfig.</rdfs:comment>
    <rdfs:domain rdf:resource="http://example.org/onto/class/google_data_loss_prevention_discovery_config"/>
    <rdfs:range rdf:resource="http://www.w3.org/2001/XMLSchema#string"/>
  </owl:DatatypeProperty>
  <owl:DatatypeProperty rdf:about="http://example.org/onto/prop/google_data_loss_prevention_discovery_config_dataset_id">
    <rdfs:label>dataset_id</rdfs:label>
    <rdfs:comment>Dataset Id of the table</rdfs:comment>
    <rdfs:domain rdf:resource="http://example.org/onto/class/google_data_loss_prevention_discovery_config"/>
    <rdfs:range rdf:resource="http://www.w3.org/2001/XMLSchema#string"/>
  </owl:DatatypeProperty>
  <owl:DatatypeProperty rdf:about="http://example.org/onto/prop/google_data_loss_prevention_discovery_config_project_id">
    <rdfs:label>project_id</rdfs:label>
    <rdfs:comment>The Google Cloud Platform project ID of the project containing the table. If omitted, the project ID is inferred from the API call.</rdfs:comment>
    <rdfs:domain rdf:resource="http://example.org/onto/class/google_data_loss_prevention_discovery_config"/>
    <rdfs:range rdf:resource="http://www.w3.org/2001/XMLSchema#string"/>
  </owl:DatatypeProperty>
  <owl:DatatypeProperty rdf:about="http://example.org/onto/prop/google_data_loss_prevention_discovery_config_table_id">
    <rdfs:label>table_id</rdfs:label>
    <rdfs:comment>Name of the table</rdfs:comment>
    <rdfs:domain rdf:resource="http://example.org/onto/class/google_data_loss_prevention_discovery_config"/>
    <rdfs:range rdf:resource="http://www.w3.org/2001/XMLSchema#string"/>
  </owl:DatatypeProperty>
  <owl:DatatypeProperty rdf:about="http://example.org/onto/prop/google_data_loss_prevention_discovery_config_detail_of_message">
    <rdfs:label>detail_of_message</rdfs:label>
    <rdfs:comment>How much data to include in the pub/sub message. Possible values: ["TABLE_PROFILE", "RESOURCE_NAME"]</rdfs:comment>
    <rdfs:domain rdf:resource="http://example.org/onto/class/google_data_loss_prevention_discovery_config"/>
    <rdfs:range rdf:resource="http://www.w3.org/2001/XMLSchema#string"/>
  </owl:DatatypeProperty>
  <owl:DatatypeProperty rdf:about="http://example.org/onto/prop/google_data_loss_prevention_discovery_config_event">
    <rdfs:label>event</rdfs:label>
    <rdfs:comment>The type of event that triggers a Pub/Sub. At most one PubSubNotification per EventType is permitted. Possible values: ["NEW_PROFILE", "CHANGED_PROFILE", "SCORE_INCREASED", "ERROR_CHANGED"]</rdfs:comment>
    <rdfs:domain rdf:resource="http://example.org/onto/class/google_data_loss_prevention_discovery_config"/>
    <rdfs:range rdf:resource="http://www.w3.org/2001/XMLSchema#string"/>
  </owl:DatatypeProperty>
  <owl:DatatypeProperty rdf:about="http://example.org/onto/prop/google_data_loss_prevention_discovery_config_topic">
    <rdfs:label>topic</rdfs:label>
    <rdfs:comment>Cloud Pub/Sub topic to send notifications to. Format is projects/{project}/topics/{topic}.</rdfs:comment>
    <rdfs:domain rdf:resource="http://example.org/onto/class/google_data_loss_prevention_discovery_config"/>
    <rdfs:range rdf:resource="http://www.w3.org/2001/XMLSchema#string"/>
  </owl:DatatypeProperty>
  <owl:DatatypeProperty rdf:about="http://example.org/onto/prop/google_data_loss_prevention_discovery_config_logical_operator">
    <rdfs:label>logical_operator</rdfs:label>
    <rdfs:comment>The operator to apply to the collection of conditions Possible values: ["OR", "AND"]</rdfs:comment>
    <rdfs:domain rdf:resource="http://example.org/onto/class/google_data_loss_prevention_discovery_config"/>
    <rdfs:range rdf:resource="http://www.w3.org/2001/XMLSchema#string"/>
  </owl:DatatypeProperty>
  <owl:DatatypeProperty rdf:about="http://example.org/onto/prop/google_data_loss_prevention_discovery_config_minimum_risk_score">
    <rdfs:label>minimum_risk_score</rdfs:label>
    <rdfs:comment>The minimum data risk score that triggers the condition. Possible values: ["HIGH", "MEDIUM_OR_HIGH"]</rdfs:comment>
    <rdfs:domain rdf:resource="http://example.org/onto/class/google_data_loss_prevention_discovery_config"/>
    <rdfs:range rdf:resource="http://www.w3.org/2001/XMLSchema#string"/>
  </owl:DatatypeProperty>
  <owl:DatatypeProperty rdf:about="http://example.org/onto/prop/google_data_loss_prevention_discovery_config_minimum_sensitivity_score">
    <rdfs:label>minimum_sensitivity_score</rdfs:label>
    <rdfs:comment>The minimum sensitivity level that triggers the condition. Possible values: ["HIGH", "MEDIUM_OR_HIGH"]</rdfs:comment>
    <rdfs:domain rdf:resource="http://example.org/onto/class/google_data_loss_prevention_discovery_config"/>
    <rdfs:range rdf:resource="http://www.w3.org/2001/XMLSchema#string"/>
  </owl:DatatypeProperty>
  <owl:DatatypeProperty rdf:about="http://example.org/onto/prop/google_data_loss_prevention_discovery_config_lower_data_risk_to_low">
    <rdfs:label>lower_data_risk_to_low</rdfs:label>
    <rdfs:comment>Whether applying a tag to a resource should lower the risk of the profile for that resource. For example, in conjunction with an [IAM deny policy](https://cloud.google.com/iam/docs/deny-overview), you can deny all principals a permission if a tag value is present, mitigating the risk of the resource. This also lowers the data risk of resources at the lower levels of the resource hierarchy. For example, reducing the data risk of a table data profile also reduces the data risk of the constituent column data profiles.</rdfs:comment>
    <rdfs:domain rdf:resource="http://example.org/onto/class/google_data_loss_prevention_discovery_config"/>
    <rdfs:range rdf:resource="http://www.w3.org/2001/XMLSchema#string"/>
  </owl:DatatypeProperty>
  <owl:DatatypeProperty rdf:about="http://example.org/onto/prop/google_data_loss_prevention_discovery_config_profile_generations_to_tag">
    <rdfs:label>profile_generations_to_tag</rdfs:label>
    <rdfs:comment>The profile generations for which the tag should be attached to resources. If you attach a tag to only new profiles, then if the sensitivity score of a profile subsequently changes, its tag doesn't change. By default, this field includes only new profiles. To include both new and updated profiles for tagging, this field should explicitly include both 'PROFILE_GENERATION_NEW' and 'PROFILE_GENERATION_UPDATE'. Possible values: ["PROFILE_GENERATION_NEW", "PROFILE_GENERATION_UPDATE"]</rdfs:comment>
    <rdfs:domain rdf:resource="http://example.org/onto/class/google_data_loss_prevention_discovery_config"/>
    <rdfs:range rdf:resource="http://www.w3.org/2001/XMLSchema#string"/>
  </owl:DatatypeProperty>
  <owl:DatatypeProperty rdf:about="http://example.org/onto/prop/google_data_loss_prevention_discovery_config_score">
    <rdfs:label>score</rdfs:label>
    <rdfs:comment>The sensitivity score applied to the resource. Possible values: ["SENSITIVITY_LOW", "SENSITIVITY_MODERATE", "SENSITIVITY_HIGH", "SENSITIVITY_UNKNOWN"]</rdfs:comment>
    <rdfs:domain rdf:resource="http://example.org/onto/class/google_data_loss_prevention_discovery_config"/>
    <rdfs:range rdf:resource="http://www.w3.org/2001/XMLSchema#string"/>
  </owl:DatatypeProperty>
  <owl:DatatypeProperty rdf:about="http://example.org/onto/prop/google_data_loss_prevention_discovery_config_namespaced_value">
    <rdfs:label>namespaced_value</rdfs:label>
    <rdfs:comment>The namespaced name for the tag value to attach to resources. Must be in the format '{parent_id}/{tag_key_short_name}/{short_name}', for example, "123456/environment/prod".</rdfs:comment>
    <rdfs:domain rdf:resource="http://example.org/onto/class/google_data_loss_prevention_discovery_config"/>
    <rdfs:range rdf:resource="http://www.w3.org/2001/XMLSchema#string"/>
  </owl:DatatypeProperty>
  <owl:DatatypeProperty rdf:about="http://example.org/onto/prop/google_data_loss_prevention_discovery_config_project_id">
    <rdfs:label>project_id</rdfs:label>
    <rdfs:comment>The project that will run the scan. The DLP service account that exists within this project must have access to all resources that are profiled, and the cloud DLP API must be enabled.</rdfs:comment>
    <rdfs:domain rdf:resource="http://example.org/onto/class/google_data_loss_prevention_discovery_config"/>
    <rdfs:range rdf:resource="http://www.w3.org/2001/XMLSchema#string"/>
  </owl:DatatypeProperty>
  <owl:DatatypeProperty rdf:about="http://example.org/onto/prop/google_data_loss_prevention_discovery_config_folder_id">
    <rdfs:label>folder_id</rdfs:label>
    <rdfs:comment>The ID for the folder within an organization to scan</rdfs:comment>
    <rdfs:domain rdf:resource="http://example.org/onto/class/google_data_loss_prevention_discovery_config"/>
    <rdfs:range rdf:resource="http://www.w3.org/2001/XMLSchema#string"/>
  </owl:DatatypeProperty>
  <owl:DatatypeProperty rdf:about="http://example.org/onto/prop/google_data_loss_prevention_discovery_config_organization_id">
    <rdfs:label>organization_id</rdfs:label>
    <rdfs:comment>The ID of an organization to scan</rdfs:comment>
    <rdfs:domain rdf:resource="http://example.org/onto/class/google_data_loss_prevention_discovery_config"/>
    <rdfs:range rdf:resource="http://www.w3.org/2001/XMLSchema#string"/>
  </owl:DatatypeProperty>
  <owl:DatatypeProperty rdf:about="http://example.org/onto/prop/google_data_loss_prevention_discovery_config_account_id">
    <rdfs:label>account_id</rdfs:label>
    <rdfs:comment>The AWS account ID that this discovery config applies to. Within an organization, you can find the AWS account ID inside an AWS account ARN. Example: arn:<partition>:organizations::<management-account-id>:account/<organization-id>/<account-id></rdfs:comment>
    <rdfs:domain rdf:resource="http://example.org/onto/class/google_data_loss_prevention_discovery_config"/>
    <rdfs:range rdf:resource="http://www.w3.org/2001/XMLSchema#string"/>
  </owl:DatatypeProperty>
  <owl:DatatypeProperty rdf:about="http://example.org/onto/prop/google_data_loss_prevention_discovery_config_all_asset_inventory_assets">
    <rdfs:label>all_asset_inventory_assets</rdfs:label>
    <rdfs:comment>All AWS assets stored in Asset Inventory that didn't match other AWS discovery configs.</rdfs:comment>
    <rdfs:domain rdf:resource="http://example.org/onto/class/google_data_loss_prevention_discovery_config"/>
    <rdfs:range rdf:resource="http://www.w3.org/2001/XMLSchema#string"/>
  </owl:DatatypeProperty>
  <owl:DatatypeProperty rdf:about="http://example.org/onto/prop/google_data_loss_prevention_discovery_config_frequency">
    <rdfs:label>frequency</rdfs:label>
    <rdfs:comment>How frequently data profiles can be updated when the template is modified. Defaults to never. Possible values: ["UPDATE_FREQUENCY_NEVER", "UPDATE_FREQUENCY_DAILY", "UPDATE_FREQUENCY_MONTHLY"]</rdfs:comment>
    <rdfs:domain rdf:resource="http://example.org/onto/class/google_data_loss_prevention_discovery_config"/>
    <rdfs:range rdf:resource="http://www.w3.org/2001/XMLSchema#string"/>
  </owl:DatatypeProperty>
  <owl:DatatypeProperty rdf:about="http://example.org/onto/prop/google_data_loss_prevention_discovery_config_frequency">
    <rdfs:label>frequency</rdfs:label>
    <rdfs:comment>How frequently profiles may be updated when schemas are modified. Default to monthly Possible values: ["UPDATE_FREQUENCY_NEVER", "UPDATE_FREQUENCY_DAILY", "UPDATE_FREQUENCY_MONTHLY"]</rdfs:comment>
    <rdfs:domain rdf:resource="http://example.org/onto/class/google_data_loss_prevention_discovery_config"/>
    <rdfs:range rdf:resource="http://www.w3.org/2001/XMLSchema#string"/>
  </owl:DatatypeProperty>
  <owl:DatatypeProperty rdf:about="http://example.org/onto/prop/google_data_loss_prevention_discovery_config_types">
    <rdfs:label>types</rdfs:label>
    <rdfs:comment>The type of events to consider when deciding if the table's schema has been modified and should have the profile updated. Defaults to NEW_COLUMN. Possible values: ["SCHEMA_NEW_COLUMNS", "SCHEMA_REMOVED_COLUMNS"]</rdfs:comment>
    <rdfs:domain rdf:resource="http://example.org/onto/class/google_data_loss_prevention_discovery_config"/>
    <rdfs:range rdf:resource="http://www.w3.org/2001/XMLSchema#string"/>
  </owl:DatatypeProperty>
  <owl:DatatypeProperty rdf:about="http://example.org/onto/prop/google_data_loss_prevention_discovery_config_frequency">
    <rdfs:label>frequency</rdfs:label>
    <rdfs:comment>How frequently data profiles can be updated when tables are modified. Defaults to never. Possible values: ["UPDATE_FREQUENCY_NEVER", "UPDATE_FREQUENCY_DAILY", "UPDATE_FREQUENCY_MONTHLY"]</rdfs:comment>
    <rdfs:domain rdf:resource="http://example.org/onto/class/google_data_loss_prevention_discovery_config"/>
    <rdfs:range rdf:resource="http://www.w3.org/2001/XMLSchema#string"/>
  </owl:DatatypeProperty>
  <owl:DatatypeProperty rdf:about="http://example.org/onto/prop/google_data_loss_prevention_discovery_config_types">
    <rdfs:label>types</rdfs:label>
    <rdfs:comment>The type of events to consider when deciding if the table has been modified and should have the profile updated. Defaults to MODIFIED_TIMESTAMP Possible values: ["TABLE_MODIFIED_TIMESTAMP"]</rdfs:comment>
    <rdfs:domain rdf:resource="http://example.org/onto/class/google_data_loss_prevention_discovery_config"/>
    <rdfs:range rdf:resource="http://www.w3.org/2001/XMLSchema#string"/>
  </owl:DatatypeProperty>
  <owl:DatatypeProperty rdf:about="http://example.org/onto/prop/google_data_loss_prevention_discovery_config_created_after">
    <rdfs:label>created_after</rdfs:label>
    <rdfs:comment>A timestamp in RFC3339 UTC "Zulu" format with nanosecond resolution and upto nine fractional digits.</rdfs:comment>
    <rdfs:domain rdf:resource="http://example.org/onto/class/google_data_loss_prevention_discovery_config"/>
    <rdfs:range rdf:resource="http://www.w3.org/2001/XMLSchema#string"/>
  </owl:DatatypeProperty>
  <owl:DatatypeProperty rdf:about="http://example.org/onto/prop/google_data_loss_prevention_discovery_config_type_collection">
    <rdfs:label>type_collection</rdfs:label>
    <rdfs:comment>Restrict discovery to categories of table types. Currently view, materialized view, snapshot and non-biglake external tables are supported. Possible values: ["BIG_QUERY_COLLECTION_ALL_TYPES", "BIG_QUERY_COLLECTION_ONLY_SUPPORTED_TYPES"]</rdfs:comment>
    <rdfs:domain rdf:resource="http://example.org/onto/class/google_data_loss_prevention_discovery_config"/>
    <rdfs:range rdf:resource="http://www.w3.org/2001/XMLSchema#string"/>
  </owl:DatatypeProperty>
  <owl:DatatypeProperty rdf:about="http://example.org/onto/prop/google_data_loss_prevention_discovery_config_min_age">
    <rdfs:label>min_age</rdfs:label>
    <rdfs:comment>Duration format. The minimum age a table must have before Cloud DLP can profile it. Value greater than 1.</rdfs:comment>
    <rdfs:domain rdf:resource="http://example.org/onto/class/google_data_loss_prevention_discovery_config"/>
    <rdfs:range rdf:resource="http://www.w3.org/2001/XMLSchema#string"/>
  </owl:DatatypeProperty>
  <owl:DatatypeProperty rdf:about="http://example.org/onto/prop/google_data_loss_prevention_discovery_config_min_row_count">
    <rdfs:label>min_row_count</rdfs:label>
    <rdfs:comment>Minimum number of rows that should be present before Cloud DLP profiles as a table.</rdfs:comment>
    <rdfs:domain rdf:resource="http://example.org/onto/class/google_data_loss_prevention_discovery_config"/>
    <rdfs:range rdf:resource="http://www.w3.org/2001/XMLSchema#string"/>
  </owl:DatatypeProperty>
  <owl:DatatypeProperty rdf:about="http://example.org/onto/prop/google_data_loss_prevention_discovery_config_types">
    <rdfs:label>types</rdfs:label>
    <rdfs:comment>A set of BiqQuery table types Possible values: ["BIG_QUERY_TABLE_TYPE_TABLE", "BIG_QUERY_TABLE_TYPE_EXTERNAL_BIG_LAKE"]</rdfs:comment>
    <rdfs:domain rdf:resource="http://example.org/onto/class/google_data_loss_prevention_discovery_config"/>
    <rdfs:range rdf:resource="http://www.w3.org/2001/XMLSchema#string"/>
  </owl:DatatypeProperty>
  <owl:DatatypeProperty rdf:about="http://example.org/onto/prop/google_data_loss_prevention_discovery_config_dataset_id">
    <rdfs:label>dataset_id</rdfs:label>
    <rdfs:comment>Dataset ID of the table.</rdfs:comment>
    <rdfs:domain rdf:resource="http://example.org/onto/class/google_data_loss_prevention_discovery_config"/>
    <rdfs:range rdf:resource="http://www.w3.org/2001/XMLSchema#string"/>
  </owl:DatatypeProperty>
  <owl:DatatypeProperty rdf:about="http://example.org/onto/prop/google_data_loss_prevention_discovery_config_table_id">
    <rdfs:label>table_id</rdfs:label>
    <rdfs:comment>Name of the table.</rdfs:comment>
    <rdfs:domain rdf:resource="http://example.org/onto/class/google_data_loss_prevention_discovery_config"/>
    <rdfs:range rdf:resource="http://www.w3.org/2001/XMLSchema#string"/>
  </owl:DatatypeProperty>
  <owl:DatatypeProperty rdf:about="http://example.org/onto/prop/google_data_loss_prevention_discovery_config_dataset_id_regex">
    <rdfs:label>dataset_id_regex</rdfs:label>
    <rdfs:comment>if unset, this property matches all datasets</rdfs:comment>
    <rdfs:domain rdf:resource="http://example.org/onto/class/google_data_loss_prevention_discovery_config"/>
    <rdfs:range rdf:resource="http://www.w3.org/2001/XMLSchema#string"/>
  </owl:DatatypeProperty>
  <owl:DatatypeProperty rdf:about="http://example.org/onto/prop/google_data_loss_prevention_discovery_config_project_id_regex">
    <rdfs:label>project_id_regex</rdfs:label>
    <rdfs:comment>For organizations, if unset, will match all projects. Has no effect for data profile configurations created within a project.</rdfs:comment>
    <rdfs:domain rdf:resource="http://example.org/onto/class/google_data_loss_prevention_discovery_config"/>
    <rdfs:range rdf:resource="http://www.w3.org/2001/XMLSchema#string"/>
  </owl:DatatypeProperty>
  <owl:DatatypeProperty rdf:about="http://example.org/onto/prop/google_data_loss_prevention_discovery_config_table_id_regex">
    <rdfs:label>table_id_regex</rdfs:label>
    <rdfs:comment>if unset, this property matches all tables</rdfs:comment>
    <rdfs:domain rdf:resource="http://example.org/onto/class/google_data_loss_prevention_discovery_config"/>
    <rdfs:range rdf:resource="http://www.w3.org/2001/XMLSchema#string"/>
  </owl:DatatypeProperty>
  <owl:DatatypeProperty rdf:about="http://example.org/onto/prop/google_data_loss_prevention_discovery_config_database_engines">
    <rdfs:label>database_engines</rdfs:label>
    <rdfs:comment>Database engines that should be profiled. Optional. Defaults to ALL_SUPPORTED_DATABASE_ENGINES if unspecified. Possible values: ["ALL_SUPPORTED_DATABASE_ENGINES", "MYSQL", "POSTGRES"]</rdfs:comment>
    <rdfs:domain rdf:resource="http://example.org/onto/class/google_data_loss_prevention_discovery_config"/>
    <rdfs:range rdf:resource="http://www.w3.org/2001/XMLSchema#string"/>
  </owl:DatatypeProperty>
  <owl:DatatypeProperty rdf:about="http://example.org/onto/prop/google_data_loss_prevention_discovery_config_types">
    <rdfs:label>types</rdfs:label>
    <rdfs:comment>Data profiles will only be generated for the database resource types specified in this field. If not specified, defaults to [DATABASE_RESOURCE_TYPE_ALL_SUPPORTED_TYPES]. Possible values: ["DATABASE_RESOURCE_TYPE_ALL_SUPPORTED_TYPES", "DATABASE_RESOURCE_TYPE_TABLE"]</rdfs:comment>
    <rdfs:domain rdf:resource="http://example.org/onto/class/google_data_loss_prevention_discovery_config"/>
    <rdfs:range rdf:resource="http://www.w3.org/2001/XMLSchema#string"/>
  </owl:DatatypeProperty>
  <owl:DatatypeProperty rdf:about="http://example.org/onto/prop/google_data_loss_prevention_discovery_config_database_regex">
    <rdfs:label>database_regex</rdfs:label>
    <rdfs:comment>Regex to test the database name against. If empty, all databases match.</rdfs:comment>
    <rdfs:domain rdf:resource="http://example.org/onto/class/google_data_loss_prevention_discovery_config"/>
    <rdfs:range rdf:resource="http://www.w3.org/2001/XMLSchema#string"/>
  </owl:DatatypeProperty>
  <owl:DatatypeProperty rdf:about="http://example.org/onto/prop/google_data_loss_prevention_discovery_config_database_resource_name_regex">
    <rdfs:label>database_resource_name_regex</rdfs:label>
    <rdfs:comment>Regex to test the database resource's name against. An example of a database resource name is a table's name. Other database resource names like view names could be included in the future. If empty, all database resources match.'</rdfs:comment>
    <rdfs:domain rdf:resource="http://example.org/onto/class/google_data_loss_prevention_discovery_config"/>
    <rdfs:range rdf:resource="http://www.w3.org/2001/XMLSchema#string"/>
  </owl:DatatypeProperty>
  <owl:DatatypeProperty rdf:about="http://example.org/onto/prop/google_data_loss_prevention_discovery_config_instance_regex">
    <rdfs:label>instance_regex</rdfs:label>
    <rdfs:comment>Regex to test the instance name against. If empty, all instances match.</rdfs:comment>
    <rdfs:domain rdf:resource="http://example.org/onto/class/google_data_loss_prevention_discovery_config"/>
    <rdfs:range rdf:resource="http://www.w3.org/2001/XMLSchema#string"/>
  </owl:DatatypeProperty>
  <owl:DatatypeProperty rdf:about="http://example.org/onto/prop/google_data_loss_prevention_discovery_config_project_id_regex">
    <rdfs:label>project_id_regex</rdfs:label>
    <rdfs:comment>For organizations, if unset, will match all projects. Has no effect for data profile configurations created within a project.</rdfs:comment>
    <rdfs:domain rdf:resource="http://example.org/onto/class/google_data_loss_prevention_discovery_config"/>
    <rdfs:range rdf:resource="http://www.w3.org/2001/XMLSchema#string"/>
  </owl:DatatypeProperty>
  <owl:DatatypeProperty rdf:about="http://example.org/onto/prop/google_data_loss_prevention_discovery_config_database">
    <rdfs:label>database</rdfs:label>
    <rdfs:comment>Required. Name of a database within the instance.</rdfs:comment>
    <rdfs:domain rdf:resource="http://example.org/onto/class/google_data_loss_prevention_discovery_config"/>
    <rdfs:range rdf:resource="http://www.w3.org/2001/XMLSchema#string"/>
  </owl:DatatypeProperty>
  <owl:DatatypeProperty rdf:about="http://example.org/onto/prop/google_data_loss_prevention_discovery_config_database_resource">
    <rdfs:label>database_resource</rdfs:label>
    <rdfs:comment>Required. Name of a database resource, for example, a table within the database.</rdfs:comment>
    <rdfs:domain rdf:resource="http://example.org/onto/class/google_data_loss_prevention_discovery_config"/>
    <rdfs:range rdf:resource="http://www.w3.org/2001/XMLSchema#string"/>
  </owl:DatatypeProperty>
  <owl:DatatypeProperty rdf:about="http://example.org/onto/prop/google_data_loss_prevention_discovery_config_instance">
    <rdfs:label>instance</rdfs:label>
    <rdfs:comment>Required. The instance where this resource is located. For example: Cloud SQL instance ID.</rdfs:comment>
    <rdfs:domain rdf:resource="http://example.org/onto/class/google_data_loss_prevention_discovery_config"/>
    <rdfs:range rdf:resource="http://www.w3.org/2001/XMLSchema#string"/>
  </owl:DatatypeProperty>
  <owl:DatatypeProperty rdf:about="http://example.org/onto/prop/google_data_loss_prevention_discovery_config_project_id">
    <rdfs:label>project_id</rdfs:label>
    <rdfs:comment>Required. If within a project-level config, then this must match the config's project ID.</rdfs:comment>
    <rdfs:domain rdf:resource="http://example.org/onto/class/google_data_loss_prevention_discovery_config"/>
    <rdfs:range rdf:resource="http://www.w3.org/2001/XMLSchema#string"/>
  </owl:DatatypeProperty>
  <owl:DatatypeProperty rdf:about="http://example.org/onto/prop/google_data_loss_prevention_discovery_config_refresh_frequency">
    <rdfs:label>refresh_frequency</rdfs:label>
    <rdfs:comment>Data changes (non-schema changes) in Cloud SQL tables can't trigger reprofiling. If you set this field, profiles are refreshed at this frequency regardless of whether the underlying tables have changes. Defaults to never. Possible values: ["UPDATE_FREQUENCY_NEVER", "UPDATE_FREQUENCY_DAILY", "UPDATE_FREQUENCY_MONTHLY"]</rdfs:comment>
    <rdfs:domain rdf:resource="http://example.org/onto/class/google_data_loss_prevention_discovery_config"/>
    <rdfs:range rdf:resource="http://www.w3.org/2001/XMLSchema#string"/>
  </owl:DatatypeProperty>
  <owl:DatatypeProperty rdf:about="http://example.org/onto/prop/google_data_loss_prevention_discovery_config_frequency">
    <rdfs:label>frequency</rdfs:label>
    <rdfs:comment>How frequently data profiles can be updated when the template is modified. Defaults to never. Possible values: ["UPDATE_FREQUENCY_NEVER", "UPDATE_FREQUENCY_DAILY", "UPDATE_FREQUENCY_MONTHLY"]</rdfs:comment>
    <rdfs:domain rdf:resource="http://example.org/onto/class/google_data_loss_prevention_discovery_config"/>
    <rdfs:range rdf:resource="http://www.w3.org/2001/XMLSchema#string"/>
  </owl:DatatypeProperty>
  <owl:DatatypeProperty rdf:about="http://example.org/onto/prop/google_data_loss_prevention_discovery_config_frequency">
    <rdfs:label>frequency</rdfs:label>
    <rdfs:comment>Frequency to regenerate data profiles when the schema is modified. Defaults to monthly. Possible values: ["UPDATE_FREQUENCY_NEVER", "UPDATE_FREQUENCY_DAILY", "UPDATE_FREQUENCY_MONTHLY"]</rdfs:comment>
    <rdfs:domain rdf:resource="http://example.org/onto/class/google_data_loss_prevention_discovery_config"/>
    <rdfs:range rdf:resource="http://www.w3.org/2001/XMLSchema#string"/>
  </owl:DatatypeProperty>
  <owl:DatatypeProperty rdf:about="http://example.org/onto/prop/google_data_loss_prevention_discovery_config_types">
    <rdfs:label>types</rdfs:label>
    <rdfs:comment>The types of schema modifications to consider. Defaults to NEW_COLUMNS. Possible values: ["NEW_COLUMNS", "REMOVED_COLUMNS"]</rdfs:comment>
    <rdfs:domain rdf:resource="http://example.org/onto/class/google_data_loss_prevention_discovery_config"/>
    <rdfs:range rdf:resource="http://www.w3.org/2001/XMLSchema#string"/>
  </owl:DatatypeProperty>
  <owl:DatatypeProperty rdf:about="http://example.org/onto/prop/google_data_loss_prevention_discovery_config_created_after">
    <rdfs:label>created_after</rdfs:label>
    <rdfs:comment>File store must have been created after this date. Used to avoid backfilling. A timestamp in RFC3339 UTC "Zulu" format with nanosecond resolution and upto nine fractional digits.</rdfs:comment>
    <rdfs:domain rdf:resource="http://example.org/onto/class/google_data_loss_prevention_discovery_config"/>
    <rdfs:range rdf:resource="http://www.w3.org/2001/XMLSchema#string"/>
  </owl:DatatypeProperty>
  <owl:DatatypeProperty rdf:about="http://example.org/onto/prop/google_data_loss_prevention_discovery_config_min_age">
    <rdfs:label>min_age</rdfs:label>
    <rdfs:comment>Duration format. Minimum age a file store must have. If set, the value must be 1 hour or greater.</rdfs:comment>
    <rdfs:domain rdf:resource="http://example.org/onto/class/google_data_loss_prevention_discovery_config"/>
    <rdfs:range rdf:resource="http://www.w3.org/2001/XMLSchema#string"/>
  </owl:DatatypeProperty>
  <owl:DatatypeProperty rdf:about="http://example.org/onto/prop/google_data_loss_prevention_discovery_config_included_bucket_attributes">
    <rdfs:label>included_bucket_attributes</rdfs:label>
    <rdfs:comment>Only objects with the specified attributes will be scanned. Defaults to [ALL_SUPPORTED_BUCKETS] if unset. Possible values: ["ALL_SUPPORTED_BUCKETS", "AUTOCLASS_DISABLED", "AUTOCLASS_ENABLED"]</rdfs:comment>
    <rdfs:domain rdf:resource="http://example.org/onto/class/google_data_loss_prevention_discovery_config"/>
    <rdfs:range rdf:resource="http://www.w3.org/2001/XMLSchema#string"/>
  </owl:DatatypeProperty>
  <owl:DatatypeProperty rdf:about="http://example.org/onto/prop/google_data_loss_prevention_discovery_config_included_object_attributes">
    <rdfs:label>included_object_attributes</rdfs:label>
    <rdfs:comment>Only objects with the specified attributes will be scanned. If an object has one of the specified attributes but is inside an excluded bucket, it will not be scanned. Defaults to [ALL_SUPPORTED_OBJECTS]. A profile will be created even if no objects match the included_object_attributes. Possible values: ["ALL_SUPPORTED_OBJECTS", "STANDARD", "NEARLINE", "COLDLINE", "ARCHIVE", "REGIONAL", "MULTI_REGIONAL", "DURABLE_REDUCED_AVAILABILITY"]</rdfs:comment>
    <rdfs:domain rdf:resource="http://example.org/onto/class/google_data_loss_prevention_discovery_config"/>
    <rdfs:range rdf:resource="http://www.w3.org/2001/XMLSchema#string"/>
  </owl:DatatypeProperty>
  <owl:DatatypeProperty rdf:about="http://example.org/onto/prop/google_data_loss_prevention_discovery_config_bucket_name">
    <rdfs:label>bucket_name</rdfs:label>
    <rdfs:comment>The bucket to scan.</rdfs:comment>
    <rdfs:domain rdf:resource="http://example.org/onto/class/google_data_loss_prevention_discovery_config"/>
    <rdfs:range rdf:resource="http://www.w3.org/2001/XMLSchema#string"/>
  </owl:DatatypeProperty>
  <owl:DatatypeProperty rdf:about="http://example.org/onto/prop/google_data_loss_prevention_discovery_config_project_id">
    <rdfs:label>project_id</rdfs:label>
    <rdfs:comment>If within a project-level config, then this must match the config's project id.</rdfs:comment>
    <rdfs:domain rdf:resource="http://example.org/onto/class/google_data_loss_prevention_discovery_config"/>
    <rdfs:range rdf:resource="http://www.w3.org/2001/XMLSchema#string"/>
  </owl:DatatypeProperty>
  <owl:DatatypeProperty rdf:about="http://example.org/onto/prop/google_data_loss_prevention_discovery_config_bucket_name_regex">
    <rdfs:label>bucket_name_regex</rdfs:label>
    <rdfs:comment>Regex to test the bucket name against. If empty, all buckets match. Example: "marketing2021" or "(marketing)\d{4}" will both match the bucket gs://marketing2021</rdfs:comment>
    <rdfs:domain rdf:resource="http://example.org/onto/class/google_data_loss_prevention_discovery_config"/>
    <rdfs:range rdf:resource="http://www.w3.org/2001/XMLSchema#string"/>
  </owl:DatatypeProperty>
  <owl:DatatypeProperty rdf:about="http://example.org/onto/prop/google_data_loss_prevention_discovery_config_project_id_regex">
    <rdfs:label>project_id_regex</rdfs:label>
    <rdfs:comment>For organizations, if unset, will match all projects.</rdfs:comment>
    <rdfs:domain rdf:resource="http://example.org/onto/class/google_data_loss_prevention_discovery_config"/>
    <rdfs:range rdf:resource="http://www.w3.org/2001/XMLSchema#string"/>
  </owl:DatatypeProperty>
  <owl:DatatypeProperty rdf:about="http://example.org/onto/prop/google_data_loss_prevention_discovery_config_refresh_frequency">
    <rdfs:label>refresh_frequency</rdfs:label>
    <rdfs:comment>Data changes in Cloud Storage can't trigger reprofiling. If you set this field, profiles are refreshed at this frequency regardless of whether the underlying buckets have changes. Defaults to never. Possible values: ["UPDATE_FREQUENCY_NEVER", "UPDATE_FREQUENCY_DAILY", "UPDATE_FREQUENCY_MONTHLY"]</rdfs:comment>
    <rdfs:domain rdf:resource="http://example.org/onto/class/google_data_loss_prevention_discovery_config"/>
    <rdfs:range rdf:resource="http://www.w3.org/2001/XMLSchema#string"/>
  </owl:DatatypeProperty>
  <owl:DatatypeProperty rdf:about="http://example.org/onto/prop/google_data_loss_prevention_discovery_config_frequency">
    <rdfs:label>frequency</rdfs:label>
    <rdfs:comment>How frequently data profiles can be updated when the template is modified. Defaults to never. Possible values: ["UPDATE_FREQUENCY_NEVER", "UPDATE_FREQUENCY_DAILY", "UPDATE_FREQUENCY_MONTHLY"]</rdfs:comment>
    <rdfs:domain rdf:resource="http://example.org/onto/class/google_data_loss_prevention_discovery_config"/>
    <rdfs:range rdf:resource="http://www.w3.org/2001/XMLSchema#string"/>
  </owl:DatatypeProperty>
  <owl:DatatypeProperty rdf:about="http://example.org/onto/prop/google_data_loss_prevention_discovery_config_min_age">
    <rdfs:label>min_age</rdfs:label>
    <rdfs:comment>Duration format.  Minimum age a resource must be before a profile can be generated. Value must be 1 hour or greater. Minimum age is not supported for Azure Blob Storage containers.</rdfs:comment>
    <rdfs:domain rdf:resource="http://example.org/onto/class/google_data_loss_prevention_discovery_config"/>
    <rdfs:range rdf:resource="http://www.w3.org/2001/XMLSchema#string"/>
  </owl:DatatypeProperty>
  <owl:DatatypeProperty rdf:about="http://example.org/onto/prop/google_data_loss_prevention_discovery_config_bucket_types">
    <rdfs:label>bucket_types</rdfs:label>
    <rdfs:comment>Bucket types that should be profiled. Optional. Defaults to TYPE_ALL_SUPPORTED if unspecified. Possible values: ["TYPE_ALL_SUPPORTED", "TYPE_GENERAL_PURPOSE"]</rdfs:comment>
    <rdfs:domain rdf:resource="http://example.org/onto/class/google_data_loss_prevention_discovery_config"/>
    <rdfs:range rdf:resource="http://www.w3.org/2001/XMLSchema#string"/>
  </owl:DatatypeProperty>
  <owl:DatatypeProperty rdf:about="http://example.org/onto/prop/google_data_loss_prevention_discovery_config_object_storage_classes">
    <rdfs:label>object_storage_classes</rdfs:label>
    <rdfs:comment>Object classes that should be profiled. Optional. Defaults to ALL_SUPPORTED_CLASSES if unspecified. Possible values: ["ALL_SUPPORTED_CLASSES", "STANDARD", "STANDARD_INFREQUENT_ACCESS", "GLACIER_INSTANT_RETRIEVAL", "INTELLIGENT_TIERING"]</rdfs:comment>
    <rdfs:domain rdf:resource="http://example.org/onto/class/google_data_loss_prevention_discovery_config"/>
    <rdfs:range rdf:resource="http://www.w3.org/2001/XMLSchema#string"/>
  </owl:DatatypeProperty>
  <owl:DatatypeProperty rdf:about="http://example.org/onto/prop/google_data_loss_prevention_discovery_config_data_source">
    <rdfs:label>data_source</rdfs:label>
    <rdfs:domain rdf:resource="http://example.org/onto/class/google_data_loss_prevention_discovery_config"/>
    <rdfs:range rdf:resource="http://www.w3.org/2001/XMLSchema#string"/>
  </owl:DatatypeProperty>
  <owl:DatatypeProperty rdf:about="http://example.org/onto/prop/google_data_loss_prevention_discovery_config_bucket_name_regex">
    <rdfs:label>bucket_name_regex</rdfs:label>
    <rdfs:comment>Regex to test the bucket name against. If empty, all buckets match.</rdfs:comment>
    <rdfs:domain rdf:resource="http://example.org/onto/class/google_data_loss_prevention_discovery_config"/>
    <rdfs:range rdf:resource="http://www.w3.org/2001/XMLSchema#string"/>
  </owl:DatatypeProperty>
  <owl:DatatypeProperty rdf:about="http://example.org/onto/prop/google_data_loss_prevention_discovery_config_account_id_regex">
    <rdfs:label>account_id_regex</rdfs:label>
    <rdfs:comment>Regex to test the AWS account ID against. If empty, all accounts match. Example: arn:aws:organizations::123:account/o-b2c3d4/345</rdfs:comment>
    <rdfs:domain rdf:resource="http://example.org/onto/class/google_data_loss_prevention_discovery_config"/>
    <rdfs:range rdf:resource="http://www.w3.org/2001/XMLSchema#string"/>
  </owl:DatatypeProperty>
  <owl:DatatypeProperty rdf:about="http://example.org/onto/prop/google_data_loss_prevention_discovery_config_bucket_name">
    <rdfs:label>bucket_name</rdfs:label>
    <rdfs:comment>The bucket name.</rdfs:comment>
    <rdfs:domain rdf:resource="http://example.org/onto/class/google_data_loss_prevention_discovery_config"/>
    <rdfs:range rdf:resource="http://www.w3.org/2001/XMLSchema#string"/>
  </owl:DatatypeProperty>
  <owl:DatatypeProperty rdf:about="http://example.org/onto/prop/google_data_loss_prevention_discovery_config_account_id">
    <rdfs:label>account_id</rdfs:label>
    <rdfs:comment>AWS account ID.</rdfs:comment>
    <rdfs:domain rdf:resource="http://example.org/onto/class/google_data_loss_prevention_discovery_config"/>
    <rdfs:range rdf:resource="http://www.w3.org/2001/XMLSchema#string"/>
  </owl:DatatypeProperty>
  <owl:DatatypeProperty rdf:about="http://example.org/onto/prop/google_data_loss_prevention_discovery_config_refresh_frequency">
    <rdfs:label>refresh_frequency</rdfs:label>
    <rdfs:comment>Frequency to update profiles regardless of whether the underlying resource has changes. Defaults to never. Possible values: ["UPDATE_FREQUENCY_NEVER", "UPDATE_FREQUENCY_DAILY", "UPDATE_FREQUENCY_MONTHLY"]</rdfs:comment>
    <rdfs:domain rdf:resource="http://example.org/onto/class/google_data_loss_prevention_discovery_config"/>
    <rdfs:range rdf:resource="http://www.w3.org/2001/XMLSchema#string"/>
  </owl:DatatypeProperty>
  <owl:DatatypeProperty rdf:about="http://example.org/onto/prop/google_data_loss_prevention_discovery_config_frequency">
    <rdfs:label>frequency</rdfs:label>
    <rdfs:comment>How frequently data profiles can be updated when the template is modified. Defaults to never. Possible values: ["UPDATE_FREQUENCY_NEVER", "UPDATE_FREQUENCY_DAILY", "UPDATE_FREQUENCY_MONTHLY"]</rdfs:comment>
    <rdfs:domain rdf:resource="http://example.org/onto/class/google_data_loss_prevention_discovery_config"/>
    <rdfs:range rdf:resource="http://www.w3.org/2001/XMLSchema#string"/>
  </owl:DatatypeProperty>
  <owl:DatatypeProperty rdf:about="http://example.org/onto/prop/google_data_loss_prevention_discovery_config_create">
    <rdfs:label>create</rdfs:label>
    <rdfs:domain rdf:resource="http://example.org/onto/class/google_data_loss_prevention_discovery_config"/>
    <rdfs:range rdf:resource="http://www.w3.org/2001/XMLSchema#string"/>
  </owl:DatatypeProperty>
  <owl:DatatypeProperty rdf:about="http://example.org/onto/prop/google_data_loss_prevention_discovery_config_delete">
    <rdfs:label>delete</rdfs:label>
    <rdfs:domain rdf:resource="http://example.org/onto/class/google_data_loss_prevention_discovery_config"/>
    <rdfs:range rdf:resource="http://www.w3.org/2001/XMLSchema#string"/>
  </owl:DatatypeProperty>
  <owl:DatatypeProperty rdf:about="http://example.org/onto/prop/google_data_loss_prevention_discovery_config_update">
    <rdfs:label>update</rdfs:label>
    <rdfs:domain rdf:resource="http://example.org/onto/class/google_data_loss_prevention_discovery_config"/>
    <rdfs:range rdf:resource="http://www.w3.org/2001/XMLSchema#string"/>
  </owl:DatatypeProperty>
</rdf:RDF>
