<?xml version="1.0" encoding="UTF-8"?>
<rdf:RDF
  xmlns:rdf="http://www.w3.org/1999/02/22-rdf-syntax-ns#"
  xmlns:rdfs="http://www.w3.org/2000/01/rdf-schema#"
  xmlns:owl="http://www.w3.org/2002/07/owl#"
  xmlns:xsd="http://www.w3.org/2001/XMLSchema#"
  xml:base="http://example.org/onto/">
  <owl:Class rdf:about="http://example.org/onto/class/google_firebase_app_hosting_backend">
    <rdfs:label>google_firebase_app_hosting_backend</rdfs:label>
    <rdfs:comment>#
#     ***     AUTO GENERATED CODE    ***    Type: MMv1     ***
#
# ----------------------------------------------------------------------------
#
#     This code is generated by Magic Modules using the following:
#
#     Configuration: https:#github.com/GoogleCloudPlatform/magic-modules/tree/main/mmv1/products/firebaseapphosting/Backend.yaml
#     Template:      https:#github.com/GoogleCloudPlatform/magic-modules/tree/main/mmv1/templates/terraform/resource.html.markdown.tmpl
#
#     DO NOT EDIT this file directly. Any changes made to this file will be
#     overwritten during the next generation cycle.
#
# ----------------------------------------------------------------------------
subcategory: "Firebase App Hosting"
description: |-
  A Backend is the primary resource of App Hosting.
---</rdfs:comment>
  </owl:Class>
  <owl:DatatypeProperty rdf:about="http://example.org/onto/prop/google_firebase_app_hosting_backend_annotations">
    <rdfs:label>annotations</rdfs:label>
    <rdfs:comment>Unstructured key value map that may be set by external tools to
store and arbitrary metadata. They are not queryable and should be
preserved when modifying objects.

**Note**: This field is non-authoritative, and will only manage the annotations present in your configuration.
Please refer to the field 'effective_annotations' for all of the annotations present on the resource.</rdfs:comment>
    <rdfs:domain rdf:resource="http://example.org/onto/class/google_firebase_app_hosting_backend"/>
    <rdfs:range rdf:resource="http://www.w3.org/2001/XMLSchema#string"/>
  </owl:DatatypeProperty>
  <owl:DatatypeProperty rdf:about="http://example.org/onto/prop/google_firebase_app_hosting_backend_app_id">
    <rdfs:label>app_id</rdfs:label>
    <rdfs:comment>The [ID of a Web
App](https://firebase.google.com/docs/reference/firebase-management/rest/v1beta1/projects.webApps#WebApp.FIELDS.app_id)
associated with the backend.</rdfs:comment>
    <rdfs:domain rdf:resource="http://example.org/onto/class/google_firebase_app_hosting_backend"/>
    <rdfs:range rdf:resource="http://www.w3.org/2001/XMLSchema#string"/>
  </owl:DatatypeProperty>
  <owl:DatatypeProperty rdf:about="http://example.org/onto/prop/google_firebase_app_hosting_backend_backend_id">
    <rdfs:label>backend_id</rdfs:label>
    <rdfs:comment>Id of the backend. Also used as the service ID for Cloud Run, and as part
of the default domain name.</rdfs:comment>
    <rdfs:domain rdf:resource="http://example.org/onto/class/google_firebase_app_hosting_backend"/>
    <rdfs:range rdf:resource="http://www.w3.org/2001/XMLSchema#string"/>
  </owl:DatatypeProperty>
  <owl:DatatypeProperty rdf:about="http://example.org/onto/prop/google_firebase_app_hosting_backend_create_time">
    <rdfs:label>create_time</rdfs:label>
    <rdfs:comment>Time at which the backend was created.</rdfs:comment>
    <rdfs:domain rdf:resource="http://example.org/onto/class/google_firebase_app_hosting_backend"/>
    <rdfs:range rdf:resource="http://www.w3.org/2001/XMLSchema#string"/>
  </owl:DatatypeProperty>
  <owl:DatatypeProperty rdf:about="http://example.org/onto/prop/google_firebase_app_hosting_backend_delete_time">
    <rdfs:label>delete_time</rdfs:label>
    <rdfs:comment>Time at which the backend was deleted.</rdfs:comment>
    <rdfs:domain rdf:resource="http://example.org/onto/class/google_firebase_app_hosting_backend"/>
    <rdfs:range rdf:resource="http://www.w3.org/2001/XMLSchema#string"/>
  </owl:DatatypeProperty>
  <owl:DatatypeProperty rdf:about="http://example.org/onto/prop/google_firebase_app_hosting_backend_display_name">
    <rdfs:label>display_name</rdfs:label>
    <rdfs:comment>Human-readable name. 63 character limit.</rdfs:comment>
    <rdfs:domain rdf:resource="http://example.org/onto/class/google_firebase_app_hosting_backend"/>
    <rdfs:range rdf:resource="http://www.w3.org/2001/XMLSchema#string"/>
  </owl:DatatypeProperty>
  <owl:DatatypeProperty rdf:about="http://example.org/onto/prop/google_firebase_app_hosting_backend_effective_annotations">
    <rdfs:label>effective_annotations</rdfs:label>
    <rdfs:comment>All of annotations (key/value pairs) present on the resource in GCP, including the annotations configured through Terraform, other clients and services.</rdfs:comment>
    <rdfs:domain rdf:resource="http://example.org/onto/class/google_firebase_app_hosting_backend"/>
    <rdfs:range rdf:resource="http://www.w3.org/2001/XMLSchema#string"/>
  </owl:DatatypeProperty>
  <owl:DatatypeProperty rdf:about="http://example.org/onto/prop/google_firebase_app_hosting_backend_effective_labels">
    <rdfs:label>effective_labels</rdfs:label>
    <rdfs:comment>All of labels (key/value pairs) present on the resource in GCP, including the labels configured through Terraform, other clients and services.</rdfs:comment>
    <rdfs:domain rdf:resource="http://example.org/onto/class/google_firebase_app_hosting_backend"/>
    <rdfs:range rdf:resource="http://www.w3.org/2001/XMLSchema#string"/>
  </owl:DatatypeProperty>
  <owl:DatatypeProperty rdf:about="http://example.org/onto/prop/google_firebase_app_hosting_backend_environment">
    <rdfs:label>environment</rdfs:label>
    <rdfs:comment>The environment name of the backend, used to load environment variables
from environment specific configuration.</rdfs:comment>
    <rdfs:domain rdf:resource="http://example.org/onto/class/google_firebase_app_hosting_backend"/>
    <rdfs:range rdf:resource="http://www.w3.org/2001/XMLSchema#string"/>
  </owl:DatatypeProperty>
  <owl:DatatypeProperty rdf:about="http://example.org/onto/prop/google_firebase_app_hosting_backend_etag">
    <rdfs:label>etag</rdfs:label>
    <rdfs:comment>Server-computed checksum based on other values; may be sent
on update or delete to ensure operation is done on expected resource.</rdfs:comment>
    <rdfs:domain rdf:resource="http://example.org/onto/class/google_firebase_app_hosting_backend"/>
    <rdfs:range rdf:resource="http://www.w3.org/2001/XMLSchema#string"/>
  </owl:DatatypeProperty>
  <owl:DatatypeProperty rdf:about="http://example.org/onto/prop/google_firebase_app_hosting_backend_id">
    <rdfs:label>id</rdfs:label>
    <rdfs:domain rdf:resource="http://example.org/onto/class/google_firebase_app_hosting_backend"/>
    <rdfs:range rdf:resource="http://www.w3.org/2001/XMLSchema#string"/>
  </owl:DatatypeProperty>
  <owl:DatatypeProperty rdf:about="http://example.org/onto/prop/google_firebase_app_hosting_backend_labels">
    <rdfs:label>labels</rdfs:label>
    <rdfs:comment>Unstructured key value map that can be used to organize and categorize
objects.

**Note**: This field is non-authoritative, and will only manage the labels present in your configuration.
Please refer to the field 'effective_labels' for all of the labels present on the resource.</rdfs:comment>
    <rdfs:domain rdf:resource="http://example.org/onto/class/google_firebase_app_hosting_backend"/>
    <rdfs:range rdf:resource="http://www.w3.org/2001/XMLSchema#string"/>
  </owl:DatatypeProperty>
  <owl:DatatypeProperty rdf:about="http://example.org/onto/prop/google_firebase_app_hosting_backend_location">
    <rdfs:label>location</rdfs:label>
    <rdfs:comment>The canonical IDs of a Google Cloud location such as "us-east1".</rdfs:comment>
    <rdfs:domain rdf:resource="http://example.org/onto/class/google_firebase_app_hosting_backend"/>
    <rdfs:range rdf:resource="http://www.w3.org/2001/XMLSchema#string"/>
  </owl:DatatypeProperty>
  <owl:DatatypeProperty rdf:about="http://example.org/onto/prop/google_firebase_app_hosting_backend_managed_resources">
    <rdfs:label>managed_resources</rdfs:label>
    <rdfs:comment>A list of the resources managed by this backend.</rdfs:comment>
    <rdfs:domain rdf:resource="http://example.org/onto/class/google_firebase_app_hosting_backend"/>
    <rdfs:range rdf:resource="http://www.w3.org/2001/XMLSchema#string"/>
  </owl:DatatypeProperty>
  <owl:DatatypeProperty rdf:about="http://example.org/onto/prop/google_firebase_app_hosting_backend_name">
    <rdfs:label>name</rdfs:label>
    <rdfs:comment>Identifier. The resource name of the backend.

Format:

'projects/{project}/locations/{locationId}/backends/{backendId}'.</rdfs:comment>
    <rdfs:domain rdf:resource="http://example.org/onto/class/google_firebase_app_hosting_backend"/>
    <rdfs:range rdf:resource="http://www.w3.org/2001/XMLSchema#string"/>
  </owl:DatatypeProperty>
  <owl:DatatypeProperty rdf:about="http://example.org/onto/prop/google_firebase_app_hosting_backend_project">
    <rdfs:label>project</rdfs:label>
    <rdfs:domain rdf:resource="http://example.org/onto/class/google_firebase_app_hosting_backend"/>
    <rdfs:range rdf:resource="http://www.w3.org/2001/XMLSchema#string"/>
  </owl:DatatypeProperty>
  <owl:DatatypeProperty rdf:about="http://example.org/onto/prop/google_firebase_app_hosting_backend_service_account">
    <rdfs:label>service_account</rdfs:label>
    <rdfs:comment>The name of the service account used for Cloud Build and Cloud Run.
Should have the role roles/firebaseapphosting.computeRunner
or equivalent permissions.</rdfs:comment>
    <rdfs:domain rdf:resource="http://example.org/onto/class/google_firebase_app_hosting_backend"/>
    <rdfs:range rdf:resource="http://www.w3.org/2001/XMLSchema#string"/>
  </owl:DatatypeProperty>
  <owl:DatatypeProperty rdf:about="http://example.org/onto/prop/google_firebase_app_hosting_backend_serving_locality">
    <rdfs:label>serving_locality</rdfs:label>
    <rdfs:comment>Immutable. Specifies how App Hosting will serve the content for this backend. It will
either be contained to a single region (REGIONAL_STRICT) or allowed to use
App Hosting's global-replicated serving infrastructure (GLOBAL_ACCESS). Possible values: ["REGIONAL_STRICT", "GLOBAL_ACCESS"]</rdfs:comment>
    <rdfs:domain rdf:resource="http://example.org/onto/class/google_firebase_app_hosting_backend"/>
    <rdfs:range rdf:resource="http://www.w3.org/2001/XMLSchema#string"/>
  </owl:DatatypeProperty>
  <owl:DatatypeProperty rdf:about="http://example.org/onto/prop/google_firebase_app_hosting_backend_terraform_labels">
    <rdfs:label>terraform_labels</rdfs:label>
    <rdfs:comment>The combination of labels configured directly on the resource
 and default labels configured on the provider.</rdfs:comment>
    <rdfs:domain rdf:resource="http://example.org/onto/class/google_firebase_app_hosting_backend"/>
    <rdfs:range rdf:resource="http://www.w3.org/2001/XMLSchema#string"/>
  </owl:DatatypeProperty>
  <owl:DatatypeProperty rdf:about="http://example.org/onto/prop/google_firebase_app_hosting_backend_uid">
    <rdfs:label>uid</rdfs:label>
    <rdfs:comment>System-assigned, unique identifier.</rdfs:comment>
    <rdfs:domain rdf:resource="http://example.org/onto/class/google_firebase_app_hosting_backend"/>
    <rdfs:range rdf:resource="http://www.w3.org/2001/XMLSchema#string"/>
  </owl:DatatypeProperty>
  <owl:DatatypeProperty rdf:about="http://example.org/onto/prop/google_firebase_app_hosting_backend_update_time">
    <rdfs:label>update_time</rdfs:label>
    <rdfs:comment>Time at which the backend was last updated.</rdfs:comment>
    <rdfs:domain rdf:resource="http://example.org/onto/class/google_firebase_app_hosting_backend"/>
    <rdfs:range rdf:resource="http://www.w3.org/2001/XMLSchema#string"/>
  </owl:DatatypeProperty>
  <owl:DatatypeProperty rdf:about="http://example.org/onto/prop/google_firebase_app_hosting_backend_uri">
    <rdfs:label>uri</rdfs:label>
    <rdfs:comment>The primary URI to communicate with the backend.</rdfs:comment>
    <rdfs:domain rdf:resource="http://example.org/onto/class/google_firebase_app_hosting_backend"/>
    <rdfs:range rdf:resource="http://www.w3.org/2001/XMLSchema#string"/>
  </owl:DatatypeProperty>
  <owl:DatatypeProperty rdf:about="http://example.org/onto/prop/google_firebase_app_hosting_backend_repository">
    <rdfs:label>repository</rdfs:label>
    <rdfs:comment>The resource name for the Developer Connect
['gitRepositoryLink'](https://cloud.google.com/developer-connect/docs/api/reference/rest/v1/projects.locations.connections.gitRepositoryLinks)
connected to this backend, in the format:

projects/{project}/locations/{location}/connections/{connection}/gitRepositoryLinks/{repositoryLink}</rdfs:comment>
    <rdfs:domain rdf:resource="http://example.org/onto/class/google_firebase_app_hosting_backend"/>
    <rdfs:range rdf:resource="http://www.w3.org/2001/XMLSchema#string"/>
  </owl:DatatypeProperty>
  <owl:DatatypeProperty rdf:about="http://example.org/onto/prop/google_firebase_app_hosting_backend_root_directory">
    <rdfs:label>root_directory</rdfs:label>
    <rdfs:comment>If 'repository' is provided, the directory relative to the root of the
repository to use as the root for the deployed web app.</rdfs:comment>
    <rdfs:domain rdf:resource="http://example.org/onto/class/google_firebase_app_hosting_backend"/>
    <rdfs:range rdf:resource="http://www.w3.org/2001/XMLSchema#string"/>
  </owl:DatatypeProperty>
  <owl:DatatypeProperty rdf:about="http://example.org/onto/prop/google_firebase_app_hosting_backend_create">
    <rdfs:label>create</rdfs:label>
    <rdfs:domain rdf:resource="http://example.org/onto/class/google_firebase_app_hosting_backend"/>
    <rdfs:range rdf:resource="http://www.w3.org/2001/XMLSchema#string"/>
  </owl:DatatypeProperty>
  <owl:DatatypeProperty rdf:about="http://example.org/onto/prop/google_firebase_app_hosting_backend_delete">
    <rdfs:label>delete</rdfs:label>
    <rdfs:domain rdf:resource="http://example.org/onto/class/google_firebase_app_hosting_backend"/>
    <rdfs:range rdf:resource="http://www.w3.org/2001/XMLSchema#string"/>
  </owl:DatatypeProperty>
  <owl:DatatypeProperty rdf:about="http://example.org/onto/prop/google_firebase_app_hosting_backend_update">
    <rdfs:label>update</rdfs:label>
    <rdfs:domain rdf:resource="http://example.org/onto/class/google_firebase_app_hosting_backend"/>
    <rdfs:range rdf:resource="http://www.w3.org/2001/XMLSchema#string"/>
  </owl:DatatypeProperty>
</rdf:RDF>
