<?xml version="1.0" encoding="UTF-8"?>
<rdf:RDF
  xmlns:rdf="http://www.w3.org/1999/02/22-rdf-syntax-ns#"
  xmlns:rdfs="http://www.w3.org/2000/01/rdf-schema#"
  xmlns:owl="http://www.w3.org/2002/07/owl#"
  xmlns:xsd="http://www.w3.org/2001/XMLSchema#"
  xml:base="http://example.org/onto/">
  <owl:Class rdf:about="http://example.org/onto/class/google_network_security_authz_policy">
    <rdfs:label>google_network_security_authz_policy</rdfs:label>
    <rdfs:comment>#
#     ***     AUTO GENERATED CODE    ***    Type: MMv1     ***
#
# ----------------------------------------------------------------------------
#
#     This code is generated by Magic Modules using the following:
#
#     Configuration: https:#github.com/GoogleCloudPlatform/magic-modules/tree/main/mmv1/products/networksecurity/AuthzPolicy.yaml
#     Template:      https:#github.com/GoogleCloudPlatform/magic-modules/tree/main/mmv1/templates/terraform/resource.html.markdown.tmpl
#
#     DO NOT EDIT this file directly. Any changes made to this file will be
#     overwritten during the next generation cycle.
#
# ----------------------------------------------------------------------------
subcategory: "Network Security"
description: |-
  AuthzPolicy is a resource that allows to forward traffic to a callout backend designed to scan the traffic for security purposes.
---</rdfs:comment>
  </owl:Class>
  <owl:DatatypeProperty rdf:about="http://example.org/onto/prop/google_network_security_authz_policy_action">
    <rdfs:label>action</rdfs:label>
    <rdfs:comment>When the action is CUSTOM, customProvider must be specified.
When the action is ALLOW, only requests matching the policy will be allowed.
When the action is DENY, only requests matching the policy will be denied.

When a request arrives, the policies are evaluated in the following order:
1. If there is a CUSTOM policy that matches the request, the CUSTOM policy is evaluated using the custom authorization providers and the request is denied if the provider rejects the request.
2. If there are any DENY policies that match the request, the request is denied.
3. If there are no ALLOW policies for the resource or if any of the ALLOW policies match the request, the request is allowed.
4. Else the request is denied by default if none of the configured AuthzPolicies with ALLOW action match the request. Possible values: ["ALLOW", "DENY", "CUSTOM"]</rdfs:comment>
    <rdfs:domain rdf:resource="http://example.org/onto/class/google_network_security_authz_policy"/>
    <rdfs:range rdf:resource="http://www.w3.org/2001/XMLSchema#string"/>
  </owl:DatatypeProperty>
  <owl:DatatypeProperty rdf:about="http://example.org/onto/prop/google_network_security_authz_policy_create_time">
    <rdfs:label>create_time</rdfs:label>
    <rdfs:comment>The timestamp when the resource was created.</rdfs:comment>
    <rdfs:domain rdf:resource="http://example.org/onto/class/google_network_security_authz_policy"/>
    <rdfs:range rdf:resource="http://www.w3.org/2001/XMLSchema#string"/>
  </owl:DatatypeProperty>
  <owl:DatatypeProperty rdf:about="http://example.org/onto/prop/google_network_security_authz_policy_description">
    <rdfs:label>description</rdfs:label>
    <rdfs:comment>A human-readable description of the resource.</rdfs:comment>
    <rdfs:domain rdf:resource="http://example.org/onto/class/google_network_security_authz_policy"/>
    <rdfs:range rdf:resource="http://www.w3.org/2001/XMLSchema#string"/>
  </owl:DatatypeProperty>
  <owl:DatatypeProperty rdf:about="http://example.org/onto/prop/google_network_security_authz_policy_effective_labels">
    <rdfs:label>effective_labels</rdfs:label>
    <rdfs:comment>All of labels (key/value pairs) present on the resource in GCP, including the labels configured through Terraform, other clients and services.</rdfs:comment>
    <rdfs:domain rdf:resource="http://example.org/onto/class/google_network_security_authz_policy"/>
    <rdfs:range rdf:resource="http://www.w3.org/2001/XMLSchema#string"/>
  </owl:DatatypeProperty>
  <owl:DatatypeProperty rdf:about="http://example.org/onto/prop/google_network_security_authz_policy_id">
    <rdfs:label>id</rdfs:label>
    <rdfs:domain rdf:resource="http://example.org/onto/class/google_network_security_authz_policy"/>
    <rdfs:range rdf:resource="http://www.w3.org/2001/XMLSchema#string"/>
  </owl:DatatypeProperty>
  <owl:DatatypeProperty rdf:about="http://example.org/onto/prop/google_network_security_authz_policy_labels">
    <rdfs:label>labels</rdfs:label>
    <rdfs:comment>Set of labels associated with the AuthzExtension resource.


**Note**: This field is non-authoritative, and will only manage the labels present in your configuration.
Please refer to the field 'effective_labels' for all of the labels present on the resource.</rdfs:comment>
    <rdfs:domain rdf:resource="http://example.org/onto/class/google_network_security_authz_policy"/>
    <rdfs:range rdf:resource="http://www.w3.org/2001/XMLSchema#string"/>
  </owl:DatatypeProperty>
  <owl:DatatypeProperty rdf:about="http://example.org/onto/prop/google_network_security_authz_policy_location">
    <rdfs:label>location</rdfs:label>
    <rdfs:comment>The location of the resource.</rdfs:comment>
    <rdfs:domain rdf:resource="http://example.org/onto/class/google_network_security_authz_policy"/>
    <rdfs:range rdf:resource="http://www.w3.org/2001/XMLSchema#string"/>
  </owl:DatatypeProperty>
  <owl:DatatypeProperty rdf:about="http://example.org/onto/prop/google_network_security_authz_policy_name">
    <rdfs:label>name</rdfs:label>
    <rdfs:comment>Identifier. Name of the AuthzPolicy resource.</rdfs:comment>
    <rdfs:domain rdf:resource="http://example.org/onto/class/google_network_security_authz_policy"/>
    <rdfs:range rdf:resource="http://www.w3.org/2001/XMLSchema#string"/>
  </owl:DatatypeProperty>
  <owl:DatatypeProperty rdf:about="http://example.org/onto/prop/google_network_security_authz_policy_project">
    <rdfs:label>project</rdfs:label>
    <rdfs:domain rdf:resource="http://example.org/onto/class/google_network_security_authz_policy"/>
    <rdfs:range rdf:resource="http://www.w3.org/2001/XMLSchema#string"/>
  </owl:DatatypeProperty>
  <owl:DatatypeProperty rdf:about="http://example.org/onto/prop/google_network_security_authz_policy_terraform_labels">
    <rdfs:label>terraform_labels</rdfs:label>
    <rdfs:comment>The combination of labels configured directly on the resource
 and default labels configured on the provider.</rdfs:comment>
    <rdfs:domain rdf:resource="http://example.org/onto/class/google_network_security_authz_policy"/>
    <rdfs:range rdf:resource="http://www.w3.org/2001/XMLSchema#string"/>
  </owl:DatatypeProperty>
  <owl:DatatypeProperty rdf:about="http://example.org/onto/prop/google_network_security_authz_policy_update_time">
    <rdfs:label>update_time</rdfs:label>
    <rdfs:comment>The timestamp when the resource was updated.</rdfs:comment>
    <rdfs:domain rdf:resource="http://example.org/onto/class/google_network_security_authz_policy"/>
    <rdfs:range rdf:resource="http://www.w3.org/2001/XMLSchema#string"/>
  </owl:DatatypeProperty>
  <owl:DatatypeProperty rdf:about="http://example.org/onto/prop/google_network_security_authz_policy_resources">
    <rdfs:label>resources</rdfs:label>
    <rdfs:comment>A list of references to authorization extensions that will be invoked for requests matching this policy. Limited to 1 custom provider.</rdfs:comment>
    <rdfs:domain rdf:resource="http://example.org/onto/class/google_network_security_authz_policy"/>
    <rdfs:range rdf:resource="http://www.w3.org/2001/XMLSchema#string"/>
  </owl:DatatypeProperty>
  <owl:DatatypeProperty rdf:about="http://example.org/onto/prop/google_network_security_authz_policy_enabled">
    <rdfs:label>enabled</rdfs:label>
    <rdfs:comment>Enable Cloud IAP at the AuthzPolicy level.</rdfs:comment>
    <rdfs:domain rdf:resource="http://example.org/onto/class/google_network_security_authz_policy"/>
    <rdfs:range rdf:resource="http://www.w3.org/2001/XMLSchema#string"/>
  </owl:DatatypeProperty>
  <owl:DatatypeProperty rdf:about="http://example.org/onto/prop/google_network_security_authz_policy_when">
    <rdfs:label>when</rdfs:label>
    <rdfs:comment>CEL expression that describes the conditions to be satisfied for the action. The result of the CEL expression is ANDed with the from and to. Refer to the CEL language reference for a list of available attributes.</rdfs:comment>
    <rdfs:domain rdf:resource="http://example.org/onto/class/google_network_security_authz_policy"/>
    <rdfs:range rdf:resource="http://www.w3.org/2001/XMLSchema#string"/>
  </owl:DatatypeProperty>
  <owl:DatatypeProperty rdf:about="http://example.org/onto/prop/google_network_security_authz_policy_length">
    <rdfs:label>length</rdfs:label>
    <rdfs:comment>The length of the address range.</rdfs:comment>
    <rdfs:domain rdf:resource="http://example.org/onto/class/google_network_security_authz_policy"/>
    <rdfs:range rdf:resource="http://www.w3.org/2001/XMLSchema#string"/>
  </owl:DatatypeProperty>
  <owl:DatatypeProperty rdf:about="http://example.org/onto/prop/google_network_security_authz_policy_prefix">
    <rdfs:label>prefix</rdfs:label>
    <rdfs:comment>The address prefix.</rdfs:comment>
    <rdfs:domain rdf:resource="http://example.org/onto/class/google_network_security_authz_policy"/>
    <rdfs:range rdf:resource="http://www.w3.org/2001/XMLSchema#string"/>
  </owl:DatatypeProperty>
  <owl:DatatypeProperty rdf:about="http://example.org/onto/prop/google_network_security_authz_policy_contains">
    <rdfs:label>contains</rdfs:label>
    <rdfs:comment>The input string must have the substring specified here. Note: empty contains match is not allowed, please use regex instead.
Examples:
* abc matches the value xyz.abc.def</rdfs:comment>
    <rdfs:domain rdf:resource="http://example.org/onto/class/google_network_security_authz_policy"/>
    <rdfs:range rdf:resource="http://www.w3.org/2001/XMLSchema#string"/>
  </owl:DatatypeProperty>
  <owl:DatatypeProperty rdf:about="http://example.org/onto/prop/google_network_security_authz_policy_exact">
    <rdfs:label>exact</rdfs:label>
    <rdfs:comment>The input string must match exactly the string specified here.
Examples:
* abc only matches the value abc.</rdfs:comment>
    <rdfs:domain rdf:resource="http://example.org/onto/class/google_network_security_authz_policy"/>
    <rdfs:range rdf:resource="http://www.w3.org/2001/XMLSchema#string"/>
  </owl:DatatypeProperty>
  <owl:DatatypeProperty rdf:about="http://example.org/onto/prop/google_network_security_authz_policy_ignore_case">
    <rdfs:label>ignore_case</rdfs:label>
    <rdfs:comment>If true, indicates the exact/prefix/suffix/contains matching should be case insensitive. For example, the matcher data will match both input string Data and data if set to true.</rdfs:comment>
    <rdfs:domain rdf:resource="http://example.org/onto/class/google_network_security_authz_policy"/>
    <rdfs:range rdf:resource="http://www.w3.org/2001/XMLSchema#string"/>
  </owl:DatatypeProperty>
  <owl:DatatypeProperty rdf:about="http://example.org/onto/prop/google_network_security_authz_policy_prefix">
    <rdfs:label>prefix</rdfs:label>
    <rdfs:comment>The input string must have the prefix specified here. Note: empty prefix is not allowed, please use regex instead.
Examples:
* abc matches the value abc.xyz</rdfs:comment>
    <rdfs:domain rdf:resource="http://example.org/onto/class/google_network_security_authz_policy"/>
    <rdfs:range rdf:resource="http://www.w3.org/2001/XMLSchema#string"/>
  </owl:DatatypeProperty>
  <owl:DatatypeProperty rdf:about="http://example.org/onto/prop/google_network_security_authz_policy_principal_selector">
    <rdfs:label>principal_selector</rdfs:label>
    <rdfs:comment>An enum to decide what principal value the principal rule will match against. If not specified, the PrincipalSelector is CLIENT_CERT_URI_SAN. Default value: "CLIENT_CERT_URI_SAN" Possible values: ["PRINCIPAL_SELECTOR_UNSPECIFIED", "CLIENT_CERT_URI_SAN", "CLIENT_CERT_DNS_NAME_SAN", "CLIENT_CERT_COMMON_NAME"]</rdfs:comment>
    <rdfs:domain rdf:resource="http://example.org/onto/class/google_network_security_authz_policy"/>
    <rdfs:range rdf:resource="http://www.w3.org/2001/XMLSchema#string"/>
  </owl:DatatypeProperty>
  <owl:DatatypeProperty rdf:about="http://example.org/onto/prop/google_network_security_authz_policy_suffix">
    <rdfs:label>suffix</rdfs:label>
    <rdfs:comment>The input string must have the suffix specified here. Note: empty prefix is not allowed, please use regex instead.
Examples:
* abc matches the value xyz.abc</rdfs:comment>
    <rdfs:domain rdf:resource="http://example.org/onto/class/google_network_security_authz_policy"/>
    <rdfs:range rdf:resource="http://www.w3.org/2001/XMLSchema#string"/>
  </owl:DatatypeProperty>
  <owl:DatatypeProperty rdf:about="http://example.org/onto/prop/google_network_security_authz_policy_contains">
    <rdfs:label>contains</rdfs:label>
    <rdfs:comment>The input string must have the substring specified here. Note: empty contains match is not allowed, please use regex instead.
Examples:
* abc matches the value xyz.abc.def</rdfs:comment>
    <rdfs:domain rdf:resource="http://example.org/onto/class/google_network_security_authz_policy"/>
    <rdfs:range rdf:resource="http://www.w3.org/2001/XMLSchema#string"/>
  </owl:DatatypeProperty>
  <owl:DatatypeProperty rdf:about="http://example.org/onto/prop/google_network_security_authz_policy_exact">
    <rdfs:label>exact</rdfs:label>
    <rdfs:comment>The input string must match exactly the string specified here.
Examples:
* abc only matches the value abc.</rdfs:comment>
    <rdfs:domain rdf:resource="http://example.org/onto/class/google_network_security_authz_policy"/>
    <rdfs:range rdf:resource="http://www.w3.org/2001/XMLSchema#string"/>
  </owl:DatatypeProperty>
  <owl:DatatypeProperty rdf:about="http://example.org/onto/prop/google_network_security_authz_policy_ignore_case">
    <rdfs:label>ignore_case</rdfs:label>
    <rdfs:comment>If true, indicates the exact/prefix/suffix/contains matching should be case insensitive. For example, the matcher data will match both input string Data and data if set to true.</rdfs:comment>
    <rdfs:domain rdf:resource="http://example.org/onto/class/google_network_security_authz_policy"/>
    <rdfs:range rdf:resource="http://www.w3.org/2001/XMLSchema#string"/>
  </owl:DatatypeProperty>
  <owl:DatatypeProperty rdf:about="http://example.org/onto/prop/google_network_security_authz_policy_prefix">
    <rdfs:label>prefix</rdfs:label>
    <rdfs:comment>The input string must have the prefix specified here. Note: empty prefix is not allowed, please use regex instead.
Examples:
* abc matches the value abc.xyz</rdfs:comment>
    <rdfs:domain rdf:resource="http://example.org/onto/class/google_network_security_authz_policy"/>
    <rdfs:range rdf:resource="http://www.w3.org/2001/XMLSchema#string"/>
  </owl:DatatypeProperty>
  <owl:DatatypeProperty rdf:about="http://example.org/onto/prop/google_network_security_authz_policy_suffix">
    <rdfs:label>suffix</rdfs:label>
    <rdfs:comment>The input string must have the suffix specified here. Note: empty prefix is not allowed, please use regex instead.
Examples:
* abc matches the value xyz.abc</rdfs:comment>
    <rdfs:domain rdf:resource="http://example.org/onto/class/google_network_security_authz_policy"/>
    <rdfs:range rdf:resource="http://www.w3.org/2001/XMLSchema#string"/>
  </owl:DatatypeProperty>
  <owl:DatatypeProperty rdf:about="http://example.org/onto/prop/google_network_security_authz_policy_contains">
    <rdfs:label>contains</rdfs:label>
    <rdfs:comment>The input string must have the substring specified here. Note: empty contains match is not allowed, please use regex instead.
Examples:
* abc matches the value xyz.abc.def</rdfs:comment>
    <rdfs:domain rdf:resource="http://example.org/onto/class/google_network_security_authz_policy"/>
    <rdfs:range rdf:resource="http://www.w3.org/2001/XMLSchema#string"/>
  </owl:DatatypeProperty>
  <owl:DatatypeProperty rdf:about="http://example.org/onto/prop/google_network_security_authz_policy_exact">
    <rdfs:label>exact</rdfs:label>
    <rdfs:comment>The input string must match exactly the string specified here.
Examples:
* abc only matches the value abc.</rdfs:comment>
    <rdfs:domain rdf:resource="http://example.org/onto/class/google_network_security_authz_policy"/>
    <rdfs:range rdf:resource="http://www.w3.org/2001/XMLSchema#string"/>
  </owl:DatatypeProperty>
  <owl:DatatypeProperty rdf:about="http://example.org/onto/prop/google_network_security_authz_policy_ignore_case">
    <rdfs:label>ignore_case</rdfs:label>
    <rdfs:comment>If true, indicates the exact/prefix/suffix/contains matching should be case insensitive. For example, the matcher data will match both input string Data and data if set to true.</rdfs:comment>
    <rdfs:domain rdf:resource="http://example.org/onto/class/google_network_security_authz_policy"/>
    <rdfs:range rdf:resource="http://www.w3.org/2001/XMLSchema#string"/>
  </owl:DatatypeProperty>
  <owl:DatatypeProperty rdf:about="http://example.org/onto/prop/google_network_security_authz_policy_prefix">
    <rdfs:label>prefix</rdfs:label>
    <rdfs:comment>The input string must have the prefix specified here. Note: empty prefix is not allowed, please use regex instead.
Examples:
* abc matches the value abc.xyz</rdfs:comment>
    <rdfs:domain rdf:resource="http://example.org/onto/class/google_network_security_authz_policy"/>
    <rdfs:range rdf:resource="http://www.w3.org/2001/XMLSchema#string"/>
  </owl:DatatypeProperty>
  <owl:DatatypeProperty rdf:about="http://example.org/onto/prop/google_network_security_authz_policy_suffix">
    <rdfs:label>suffix</rdfs:label>
    <rdfs:comment>The input string must have the suffix specified here. Note: empty prefix is not allowed, please use regex instead.
Examples:
* abc matches the value xyz.abc</rdfs:comment>
    <rdfs:domain rdf:resource="http://example.org/onto/class/google_network_security_authz_policy"/>
    <rdfs:range rdf:resource="http://www.w3.org/2001/XMLSchema#string"/>
  </owl:DatatypeProperty>
  <owl:DatatypeProperty rdf:about="http://example.org/onto/prop/google_network_security_authz_policy_ids">
    <rdfs:label>ids</rdfs:label>
    <rdfs:comment>A list of resource tag value permanent IDs to match against the resource manager tags value associated with the source VM of a request. The match follows AND semantics which means all the ids must match.
Limited to 5 matches.</rdfs:comment>
    <rdfs:domain rdf:resource="http://example.org/onto/class/google_network_security_authz_policy"/>
    <rdfs:range rdf:resource="http://www.w3.org/2001/XMLSchema#string"/>
  </owl:DatatypeProperty>
  <owl:DatatypeProperty rdf:about="http://example.org/onto/prop/google_network_security_authz_policy_length">
    <rdfs:label>length</rdfs:label>
    <rdfs:comment>The length of the address range.</rdfs:comment>
    <rdfs:domain rdf:resource="http://example.org/onto/class/google_network_security_authz_policy"/>
    <rdfs:range rdf:resource="http://www.w3.org/2001/XMLSchema#string"/>
  </owl:DatatypeProperty>
  <owl:DatatypeProperty rdf:about="http://example.org/onto/prop/google_network_security_authz_policy_prefix">
    <rdfs:label>prefix</rdfs:label>
    <rdfs:comment>The address prefix.</rdfs:comment>
    <rdfs:domain rdf:resource="http://example.org/onto/class/google_network_security_authz_policy"/>
    <rdfs:range rdf:resource="http://www.w3.org/2001/XMLSchema#string"/>
  </owl:DatatypeProperty>
  <owl:DatatypeProperty rdf:about="http://example.org/onto/prop/google_network_security_authz_policy_contains">
    <rdfs:label>contains</rdfs:label>
    <rdfs:comment>The input string must have the substring specified here. Note: empty contains match is not allowed, please use regex instead.
Examples:
* abc matches the value xyz.abc.def</rdfs:comment>
    <rdfs:domain rdf:resource="http://example.org/onto/class/google_network_security_authz_policy"/>
    <rdfs:range rdf:resource="http://www.w3.org/2001/XMLSchema#string"/>
  </owl:DatatypeProperty>
  <owl:DatatypeProperty rdf:about="http://example.org/onto/prop/google_network_security_authz_policy_exact">
    <rdfs:label>exact</rdfs:label>
    <rdfs:comment>The input string must match exactly the string specified here.
Examples:
* abc only matches the value abc.</rdfs:comment>
    <rdfs:domain rdf:resource="http://example.org/onto/class/google_network_security_authz_policy"/>
    <rdfs:range rdf:resource="http://www.w3.org/2001/XMLSchema#string"/>
  </owl:DatatypeProperty>
  <owl:DatatypeProperty rdf:about="http://example.org/onto/prop/google_network_security_authz_policy_ignore_case">
    <rdfs:label>ignore_case</rdfs:label>
    <rdfs:comment>If true, indicates the exact/prefix/suffix/contains matching should be case insensitive. For example, the matcher data will match both input string Data and data if set to true.</rdfs:comment>
    <rdfs:domain rdf:resource="http://example.org/onto/class/google_network_security_authz_policy"/>
    <rdfs:range rdf:resource="http://www.w3.org/2001/XMLSchema#string"/>
  </owl:DatatypeProperty>
  <owl:DatatypeProperty rdf:about="http://example.org/onto/prop/google_network_security_authz_policy_prefix">
    <rdfs:label>prefix</rdfs:label>
    <rdfs:comment>The input string must have the prefix specified here. Note: empty prefix is not allowed, please use regex instead.
Examples:
* abc matches the value abc.xyz</rdfs:comment>
    <rdfs:domain rdf:resource="http://example.org/onto/class/google_network_security_authz_policy"/>
    <rdfs:range rdf:resource="http://www.w3.org/2001/XMLSchema#string"/>
  </owl:DatatypeProperty>
  <owl:DatatypeProperty rdf:about="http://example.org/onto/prop/google_network_security_authz_policy_principal_selector">
    <rdfs:label>principal_selector</rdfs:label>
    <rdfs:comment>An enum to decide what principal value the principal rule will match against. If not specified, the PrincipalSelector is CLIENT_CERT_URI_SAN. Default value: "CLIENT_CERT_URI_SAN" Possible values: ["PRINCIPAL_SELECTOR_UNSPECIFIED", "CLIENT_CERT_URI_SAN", "CLIENT_CERT_DNS_NAME_SAN", "CLIENT_CERT_COMMON_NAME"]</rdfs:comment>
    <rdfs:domain rdf:resource="http://example.org/onto/class/google_network_security_authz_policy"/>
    <rdfs:range rdf:resource="http://www.w3.org/2001/XMLSchema#string"/>
  </owl:DatatypeProperty>
  <owl:DatatypeProperty rdf:about="http://example.org/onto/prop/google_network_security_authz_policy_suffix">
    <rdfs:label>suffix</rdfs:label>
    <rdfs:comment>The input string must have the suffix specified here. Note: empty prefix is not allowed, please use regex instead.
Examples:
* abc matches the value xyz.abc</rdfs:comment>
    <rdfs:domain rdf:resource="http://example.org/onto/class/google_network_security_authz_policy"/>
    <rdfs:range rdf:resource="http://www.w3.org/2001/XMLSchema#string"/>
  </owl:DatatypeProperty>
  <owl:DatatypeProperty rdf:about="http://example.org/onto/prop/google_network_security_authz_policy_contains">
    <rdfs:label>contains</rdfs:label>
    <rdfs:comment>The input string must have the substring specified here. Note: empty contains match is not allowed, please use regex instead.
Examples:
* abc matches the value xyz.abc.def</rdfs:comment>
    <rdfs:domain rdf:resource="http://example.org/onto/class/google_network_security_authz_policy"/>
    <rdfs:range rdf:resource="http://www.w3.org/2001/XMLSchema#string"/>
  </owl:DatatypeProperty>
  <owl:DatatypeProperty rdf:about="http://example.org/onto/prop/google_network_security_authz_policy_exact">
    <rdfs:label>exact</rdfs:label>
    <rdfs:comment>The input string must match exactly the string specified here.
Examples:
* abc only matches the value abc.</rdfs:comment>
    <rdfs:domain rdf:resource="http://example.org/onto/class/google_network_security_authz_policy"/>
    <rdfs:range rdf:resource="http://www.w3.org/2001/XMLSchema#string"/>
  </owl:DatatypeProperty>
  <owl:DatatypeProperty rdf:about="http://example.org/onto/prop/google_network_security_authz_policy_ignore_case">
    <rdfs:label>ignore_case</rdfs:label>
    <rdfs:comment>If true, indicates the exact/prefix/suffix/contains matching should be case insensitive. For example, the matcher data will match both input string Data and data if set to true.</rdfs:comment>
    <rdfs:domain rdf:resource="http://example.org/onto/class/google_network_security_authz_policy"/>
    <rdfs:range rdf:resource="http://www.w3.org/2001/XMLSchema#string"/>
  </owl:DatatypeProperty>
  <owl:DatatypeProperty rdf:about="http://example.org/onto/prop/google_network_security_authz_policy_prefix">
    <rdfs:label>prefix</rdfs:label>
    <rdfs:comment>The input string must have the prefix specified here. Note: empty prefix is not allowed, please use regex instead.
Examples:
* abc matches the value abc.xyz</rdfs:comment>
    <rdfs:domain rdf:resource="http://example.org/onto/class/google_network_security_authz_policy"/>
    <rdfs:range rdf:resource="http://www.w3.org/2001/XMLSchema#string"/>
  </owl:DatatypeProperty>
  <owl:DatatypeProperty rdf:about="http://example.org/onto/prop/google_network_security_authz_policy_suffix">
    <rdfs:label>suffix</rdfs:label>
    <rdfs:comment>The input string must have the suffix specified here. Note: empty prefix is not allowed, please use regex instead.
Examples:
* abc matches the value xyz.abc</rdfs:comment>
    <rdfs:domain rdf:resource="http://example.org/onto/class/google_network_security_authz_policy"/>
    <rdfs:range rdf:resource="http://www.w3.org/2001/XMLSchema#string"/>
  </owl:DatatypeProperty>
  <owl:DatatypeProperty rdf:about="http://example.org/onto/prop/google_network_security_authz_policy_contains">
    <rdfs:label>contains</rdfs:label>
    <rdfs:comment>The input string must have the substring specified here. Note: empty contains match is not allowed, please use regex instead.
Examples:
* abc matches the value xyz.abc.def</rdfs:comment>
    <rdfs:domain rdf:resource="http://example.org/onto/class/google_network_security_authz_policy"/>
    <rdfs:range rdf:resource="http://www.w3.org/2001/XMLSchema#string"/>
  </owl:DatatypeProperty>
  <owl:DatatypeProperty rdf:about="http://example.org/onto/prop/google_network_security_authz_policy_exact">
    <rdfs:label>exact</rdfs:label>
    <rdfs:comment>The input string must match exactly the string specified here.
Examples:
* abc only matches the value abc.</rdfs:comment>
    <rdfs:domain rdf:resource="http://example.org/onto/class/google_network_security_authz_policy"/>
    <rdfs:range rdf:resource="http://www.w3.org/2001/XMLSchema#string"/>
  </owl:DatatypeProperty>
  <owl:DatatypeProperty rdf:about="http://example.org/onto/prop/google_network_security_authz_policy_ignore_case">
    <rdfs:label>ignore_case</rdfs:label>
    <rdfs:comment>If true, indicates the exact/prefix/suffix/contains matching should be case insensitive. For example, the matcher data will match both input string Data and data if set to true.</rdfs:comment>
    <rdfs:domain rdf:resource="http://example.org/onto/class/google_network_security_authz_policy"/>
    <rdfs:range rdf:resource="http://www.w3.org/2001/XMLSchema#string"/>
  </owl:DatatypeProperty>
  <owl:DatatypeProperty rdf:about="http://example.org/onto/prop/google_network_security_authz_policy_prefix">
    <rdfs:label>prefix</rdfs:label>
    <rdfs:comment>The input string must have the prefix specified here. Note: empty prefix is not allowed, please use regex instead.
Examples:
* abc matches the value abc.xyz</rdfs:comment>
    <rdfs:domain rdf:resource="http://example.org/onto/class/google_network_security_authz_policy"/>
    <rdfs:range rdf:resource="http://www.w3.org/2001/XMLSchema#string"/>
  </owl:DatatypeProperty>
  <owl:DatatypeProperty rdf:about="http://example.org/onto/prop/google_network_security_authz_policy_suffix">
    <rdfs:label>suffix</rdfs:label>
    <rdfs:comment>The input string must have the suffix specified here. Note: empty prefix is not allowed, please use regex instead.
Examples:
* abc matches the value xyz.abc</rdfs:comment>
    <rdfs:domain rdf:resource="http://example.org/onto/class/google_network_security_authz_policy"/>
    <rdfs:range rdf:resource="http://www.w3.org/2001/XMLSchema#string"/>
  </owl:DatatypeProperty>
  <owl:DatatypeProperty rdf:about="http://example.org/onto/prop/google_network_security_authz_policy_ids">
    <rdfs:label>ids</rdfs:label>
    <rdfs:comment>A list of resource tag value permanent IDs to match against the resource manager tags value associated with the source VM of a request. The match follows AND semantics which means all the ids must match.
Limited to 5 matches.</rdfs:comment>
    <rdfs:domain rdf:resource="http://example.org/onto/class/google_network_security_authz_policy"/>
    <rdfs:range rdf:resource="http://www.w3.org/2001/XMLSchema#string"/>
  </owl:DatatypeProperty>
  <owl:DatatypeProperty rdf:about="http://example.org/onto/prop/google_network_security_authz_policy_methods">
    <rdfs:label>methods</rdfs:label>
    <rdfs:comment>A list of HTTP methods to match against. Each entry must be a valid HTTP method name (GET, PUT, POST, HEAD, PATCH, DELETE, OPTIONS). It only allows exact match and is always case sensitive.</rdfs:comment>
    <rdfs:domain rdf:resource="http://example.org/onto/class/google_network_security_authz_policy"/>
    <rdfs:range rdf:resource="http://www.w3.org/2001/XMLSchema#string"/>
  </owl:DatatypeProperty>
  <owl:DatatypeProperty rdf:about="http://example.org/onto/prop/google_network_security_authz_policy_name">
    <rdfs:label>name</rdfs:label>
    <rdfs:comment>Specifies the name of the header in the request.</rdfs:comment>
    <rdfs:domain rdf:resource="http://example.org/onto/class/google_network_security_authz_policy"/>
    <rdfs:range rdf:resource="http://www.w3.org/2001/XMLSchema#string"/>
  </owl:DatatypeProperty>
  <owl:DatatypeProperty rdf:about="http://example.org/onto/prop/google_network_security_authz_policy_contains">
    <rdfs:label>contains</rdfs:label>
    <rdfs:comment>The input string must have the substring specified here. Note: empty contains match is not allowed, please use regex instead.
Examples:
* abc matches the value xyz.abc.def</rdfs:comment>
    <rdfs:domain rdf:resource="http://example.org/onto/class/google_network_security_authz_policy"/>
    <rdfs:range rdf:resource="http://www.w3.org/2001/XMLSchema#string"/>
  </owl:DatatypeProperty>
  <owl:DatatypeProperty rdf:about="http://example.org/onto/prop/google_network_security_authz_policy_exact">
    <rdfs:label>exact</rdfs:label>
    <rdfs:comment>The input string must match exactly the string specified here.
Examples:
* abc only matches the value abc.</rdfs:comment>
    <rdfs:domain rdf:resource="http://example.org/onto/class/google_network_security_authz_policy"/>
    <rdfs:range rdf:resource="http://www.w3.org/2001/XMLSchema#string"/>
  </owl:DatatypeProperty>
  <owl:DatatypeProperty rdf:about="http://example.org/onto/prop/google_network_security_authz_policy_ignore_case">
    <rdfs:label>ignore_case</rdfs:label>
    <rdfs:comment>If true, indicates the exact/prefix/suffix/contains matching should be case insensitive. For example, the matcher data will match both input string Data and data if set to true.</rdfs:comment>
    <rdfs:domain rdf:resource="http://example.org/onto/class/google_network_security_authz_policy"/>
    <rdfs:range rdf:resource="http://www.w3.org/2001/XMLSchema#string"/>
  </owl:DatatypeProperty>
  <owl:DatatypeProperty rdf:about="http://example.org/onto/prop/google_network_security_authz_policy_prefix">
    <rdfs:label>prefix</rdfs:label>
    <rdfs:comment>The input string must have the prefix specified here. Note: empty prefix is not allowed, please use regex instead.
Examples:
* abc matches the value abc.xyz</rdfs:comment>
    <rdfs:domain rdf:resource="http://example.org/onto/class/google_network_security_authz_policy"/>
    <rdfs:range rdf:resource="http://www.w3.org/2001/XMLSchema#string"/>
  </owl:DatatypeProperty>
  <owl:DatatypeProperty rdf:about="http://example.org/onto/prop/google_network_security_authz_policy_suffix">
    <rdfs:label>suffix</rdfs:label>
    <rdfs:comment>The input string must have the suffix specified here. Note: empty prefix is not allowed, please use regex instead.
Examples:
* abc matches the value xyz.abc</rdfs:comment>
    <rdfs:domain rdf:resource="http://example.org/onto/class/google_network_security_authz_policy"/>
    <rdfs:range rdf:resource="http://www.w3.org/2001/XMLSchema#string"/>
  </owl:DatatypeProperty>
  <owl:DatatypeProperty rdf:about="http://example.org/onto/prop/google_network_security_authz_policy_contains">
    <rdfs:label>contains</rdfs:label>
    <rdfs:comment>The input string must have the substring specified here. Note: empty contains match is not allowed, please use regex instead.
Examples:
* abc matches the value xyz.abc.def</rdfs:comment>
    <rdfs:domain rdf:resource="http://example.org/onto/class/google_network_security_authz_policy"/>
    <rdfs:range rdf:resource="http://www.w3.org/2001/XMLSchema#string"/>
  </owl:DatatypeProperty>
  <owl:DatatypeProperty rdf:about="http://example.org/onto/prop/google_network_security_authz_policy_exact">
    <rdfs:label>exact</rdfs:label>
    <rdfs:comment>The input string must match exactly the string specified here.
Examples:
* abc only matches the value abc.</rdfs:comment>
    <rdfs:domain rdf:resource="http://example.org/onto/class/google_network_security_authz_policy"/>
    <rdfs:range rdf:resource="http://www.w3.org/2001/XMLSchema#string"/>
  </owl:DatatypeProperty>
  <owl:DatatypeProperty rdf:about="http://example.org/onto/prop/google_network_security_authz_policy_ignore_case">
    <rdfs:label>ignore_case</rdfs:label>
    <rdfs:comment>If true, indicates the exact/prefix/suffix/contains matching should be case insensitive. For example, the matcher data will match both input string Data and data if set to true.</rdfs:comment>
    <rdfs:domain rdf:resource="http://example.org/onto/class/google_network_security_authz_policy"/>
    <rdfs:range rdf:resource="http://www.w3.org/2001/XMLSchema#string"/>
  </owl:DatatypeProperty>
  <owl:DatatypeProperty rdf:about="http://example.org/onto/prop/google_network_security_authz_policy_prefix">
    <rdfs:label>prefix</rdfs:label>
    <rdfs:comment>The input string must have the prefix specified here. Note: empty prefix is not allowed, please use regex instead.
Examples:
* abc matches the value abc.xyz</rdfs:comment>
    <rdfs:domain rdf:resource="http://example.org/onto/class/google_network_security_authz_policy"/>
    <rdfs:range rdf:resource="http://www.w3.org/2001/XMLSchema#string"/>
  </owl:DatatypeProperty>
  <owl:DatatypeProperty rdf:about="http://example.org/onto/prop/google_network_security_authz_policy_suffix">
    <rdfs:label>suffix</rdfs:label>
    <rdfs:comment>The input string must have the suffix specified here. Note: empty prefix is not allowed, please use regex instead.
Examples:
* abc matches the value xyz.abc</rdfs:comment>
    <rdfs:domain rdf:resource="http://example.org/onto/class/google_network_security_authz_policy"/>
    <rdfs:range rdf:resource="http://www.w3.org/2001/XMLSchema#string"/>
  </owl:DatatypeProperty>
  <owl:DatatypeProperty rdf:about="http://example.org/onto/prop/google_network_security_authz_policy_contains">
    <rdfs:label>contains</rdfs:label>
    <rdfs:comment>The input string must have the substring specified here. Note: empty contains match is not allowed, please use regex instead.
Examples:
* abc matches the value xyz.abc.def</rdfs:comment>
    <rdfs:domain rdf:resource="http://example.org/onto/class/google_network_security_authz_policy"/>
    <rdfs:range rdf:resource="http://www.w3.org/2001/XMLSchema#string"/>
  </owl:DatatypeProperty>
  <owl:DatatypeProperty rdf:about="http://example.org/onto/prop/google_network_security_authz_policy_exact">
    <rdfs:label>exact</rdfs:label>
    <rdfs:comment>The input string must match exactly the string specified here.
Examples:
* abc only matches the value abc.</rdfs:comment>
    <rdfs:domain rdf:resource="http://example.org/onto/class/google_network_security_authz_policy"/>
    <rdfs:range rdf:resource="http://www.w3.org/2001/XMLSchema#string"/>
  </owl:DatatypeProperty>
  <owl:DatatypeProperty rdf:about="http://example.org/onto/prop/google_network_security_authz_policy_ignore_case">
    <rdfs:label>ignore_case</rdfs:label>
    <rdfs:comment>If true, indicates the exact/prefix/suffix/contains matching should be case insensitive. For example, the matcher data will match both input string Data and data if set to true.</rdfs:comment>
    <rdfs:domain rdf:resource="http://example.org/onto/class/google_network_security_authz_policy"/>
    <rdfs:range rdf:resource="http://www.w3.org/2001/XMLSchema#string"/>
  </owl:DatatypeProperty>
  <owl:DatatypeProperty rdf:about="http://example.org/onto/prop/google_network_security_authz_policy_prefix">
    <rdfs:label>prefix</rdfs:label>
    <rdfs:comment>The input string must have the prefix specified here. Note: empty prefix is not allowed, please use regex instead.
Examples:
* abc matches the value abc.xyz</rdfs:comment>
    <rdfs:domain rdf:resource="http://example.org/onto/class/google_network_security_authz_policy"/>
    <rdfs:range rdf:resource="http://www.w3.org/2001/XMLSchema#string"/>
  </owl:DatatypeProperty>
  <owl:DatatypeProperty rdf:about="http://example.org/onto/prop/google_network_security_authz_policy_suffix">
    <rdfs:label>suffix</rdfs:label>
    <rdfs:comment>The input string must have the suffix specified here. Note: empty prefix is not allowed, please use regex instead.
Examples:
* abc matches the value xyz.abc</rdfs:comment>
    <rdfs:domain rdf:resource="http://example.org/onto/class/google_network_security_authz_policy"/>
    <rdfs:range rdf:resource="http://www.w3.org/2001/XMLSchema#string"/>
  </owl:DatatypeProperty>
  <owl:DatatypeProperty rdf:about="http://example.org/onto/prop/google_network_security_authz_policy_methods">
    <rdfs:label>methods</rdfs:label>
    <rdfs:comment>A list of HTTP methods to match against. Each entry must be a valid HTTP method name (GET, PUT, POST, HEAD, PATCH, DELETE, OPTIONS). It only allows exact match and is always case sensitive.</rdfs:comment>
    <rdfs:domain rdf:resource="http://example.org/onto/class/google_network_security_authz_policy"/>
    <rdfs:range rdf:resource="http://www.w3.org/2001/XMLSchema#string"/>
  </owl:DatatypeProperty>
  <owl:DatatypeProperty rdf:about="http://example.org/onto/prop/google_network_security_authz_policy_name">
    <rdfs:label>name</rdfs:label>
    <rdfs:comment>Specifies the name of the header in the request.</rdfs:comment>
    <rdfs:domain rdf:resource="http://example.org/onto/class/google_network_security_authz_policy"/>
    <rdfs:range rdf:resource="http://www.w3.org/2001/XMLSchema#string"/>
  </owl:DatatypeProperty>
  <owl:DatatypeProperty rdf:about="http://example.org/onto/prop/google_network_security_authz_policy_contains">
    <rdfs:label>contains</rdfs:label>
    <rdfs:comment>The input string must have the substring specified here. Note: empty contains match is not allowed, please use regex instead.
Examples:
* abc matches the value xyz.abc.def</rdfs:comment>
    <rdfs:domain rdf:resource="http://example.org/onto/class/google_network_security_authz_policy"/>
    <rdfs:range rdf:resource="http://www.w3.org/2001/XMLSchema#string"/>
  </owl:DatatypeProperty>
  <owl:DatatypeProperty rdf:about="http://example.org/onto/prop/google_network_security_authz_policy_exact">
    <rdfs:label>exact</rdfs:label>
    <rdfs:comment>The input string must match exactly the string specified here.
Examples:
* abc only matches the value abc.</rdfs:comment>
    <rdfs:domain rdf:resource="http://example.org/onto/class/google_network_security_authz_policy"/>
    <rdfs:range rdf:resource="http://www.w3.org/2001/XMLSchema#string"/>
  </owl:DatatypeProperty>
  <owl:DatatypeProperty rdf:about="http://example.org/onto/prop/google_network_security_authz_policy_ignore_case">
    <rdfs:label>ignore_case</rdfs:label>
    <rdfs:comment>If true, indicates the exact/prefix/suffix/contains matching should be case insensitive. For example, the matcher data will match both input string Data and data if set to true.</rdfs:comment>
    <rdfs:domain rdf:resource="http://example.org/onto/class/google_network_security_authz_policy"/>
    <rdfs:range rdf:resource="http://www.w3.org/2001/XMLSchema#string"/>
  </owl:DatatypeProperty>
  <owl:DatatypeProperty rdf:about="http://example.org/onto/prop/google_network_security_authz_policy_prefix">
    <rdfs:label>prefix</rdfs:label>
    <rdfs:comment>The input string must have the prefix specified here. Note: empty prefix is not allowed, please use regex instead.
Examples:
* abc matches the value abc.xyz</rdfs:comment>
    <rdfs:domain rdf:resource="http://example.org/onto/class/google_network_security_authz_policy"/>
    <rdfs:range rdf:resource="http://www.w3.org/2001/XMLSchema#string"/>
  </owl:DatatypeProperty>
  <owl:DatatypeProperty rdf:about="http://example.org/onto/prop/google_network_security_authz_policy_suffix">
    <rdfs:label>suffix</rdfs:label>
    <rdfs:comment>The input string must have the suffix specified here. Note: empty prefix is not allowed, please use regex instead.
Examples:
* abc matches the value xyz.abc</rdfs:comment>
    <rdfs:domain rdf:resource="http://example.org/onto/class/google_network_security_authz_policy"/>
    <rdfs:range rdf:resource="http://www.w3.org/2001/XMLSchema#string"/>
  </owl:DatatypeProperty>
  <owl:DatatypeProperty rdf:about="http://example.org/onto/prop/google_network_security_authz_policy_contains">
    <rdfs:label>contains</rdfs:label>
    <rdfs:comment>The input string must have the substring specified here. Note: empty contains match is not allowed, please use regex instead.
Examples:
* abc matches the value xyz.abc.def</rdfs:comment>
    <rdfs:domain rdf:resource="http://example.org/onto/class/google_network_security_authz_policy"/>
    <rdfs:range rdf:resource="http://www.w3.org/2001/XMLSchema#string"/>
  </owl:DatatypeProperty>
  <owl:DatatypeProperty rdf:about="http://example.org/onto/prop/google_network_security_authz_policy_exact">
    <rdfs:label>exact</rdfs:label>
    <rdfs:comment>The input string must match exactly the string specified here.
Examples:
* abc only matches the value abc.</rdfs:comment>
    <rdfs:domain rdf:resource="http://example.org/onto/class/google_network_security_authz_policy"/>
    <rdfs:range rdf:resource="http://www.w3.org/2001/XMLSchema#string"/>
  </owl:DatatypeProperty>
  <owl:DatatypeProperty rdf:about="http://example.org/onto/prop/google_network_security_authz_policy_ignore_case">
    <rdfs:label>ignore_case</rdfs:label>
    <rdfs:comment>If true, indicates the exact/prefix/suffix/contains matching should be case insensitive. For example, the matcher data will match both input string Data and data if set to true.</rdfs:comment>
    <rdfs:domain rdf:resource="http://example.org/onto/class/google_network_security_authz_policy"/>
    <rdfs:range rdf:resource="http://www.w3.org/2001/XMLSchema#string"/>
  </owl:DatatypeProperty>
  <owl:DatatypeProperty rdf:about="http://example.org/onto/prop/google_network_security_authz_policy_prefix">
    <rdfs:label>prefix</rdfs:label>
    <rdfs:comment>The input string must have the prefix specified here. Note: empty prefix is not allowed, please use regex instead.
Examples:
* abc matches the value abc.xyz</rdfs:comment>
    <rdfs:domain rdf:resource="http://example.org/onto/class/google_network_security_authz_policy"/>
    <rdfs:range rdf:resource="http://www.w3.org/2001/XMLSchema#string"/>
  </owl:DatatypeProperty>
  <owl:DatatypeProperty rdf:about="http://example.org/onto/prop/google_network_security_authz_policy_suffix">
    <rdfs:label>suffix</rdfs:label>
    <rdfs:comment>The input string must have the suffix specified here. Note: empty prefix is not allowed, please use regex instead.
Examples:
* abc matches the value xyz.abc</rdfs:comment>
    <rdfs:domain rdf:resource="http://example.org/onto/class/google_network_security_authz_policy"/>
    <rdfs:range rdf:resource="http://www.w3.org/2001/XMLSchema#string"/>
  </owl:DatatypeProperty>
  <owl:DatatypeProperty rdf:about="http://example.org/onto/prop/google_network_security_authz_policy_contains">
    <rdfs:label>contains</rdfs:label>
    <rdfs:comment>The input string must have the substring specified here. Note: empty contains match is not allowed, please use regex instead.
Examples:
* abc matches the value xyz.abc.def</rdfs:comment>
    <rdfs:domain rdf:resource="http://example.org/onto/class/google_network_security_authz_policy"/>
    <rdfs:range rdf:resource="http://www.w3.org/2001/XMLSchema#string"/>
  </owl:DatatypeProperty>
  <owl:DatatypeProperty rdf:about="http://example.org/onto/prop/google_network_security_authz_policy_exact">
    <rdfs:label>exact</rdfs:label>
    <rdfs:comment>The input string must match exactly the string specified here.
Examples:
* abc only matches the value abc.</rdfs:comment>
    <rdfs:domain rdf:resource="http://example.org/onto/class/google_network_security_authz_policy"/>
    <rdfs:range rdf:resource="http://www.w3.org/2001/XMLSchema#string"/>
  </owl:DatatypeProperty>
  <owl:DatatypeProperty rdf:about="http://example.org/onto/prop/google_network_security_authz_policy_ignore_case">
    <rdfs:label>ignore_case</rdfs:label>
    <rdfs:comment>If true, indicates the exact/prefix/suffix/contains matching should be case insensitive. For example, the matcher data will match both input string Data and data if set to true.</rdfs:comment>
    <rdfs:domain rdf:resource="http://example.org/onto/class/google_network_security_authz_policy"/>
    <rdfs:range rdf:resource="http://www.w3.org/2001/XMLSchema#string"/>
  </owl:DatatypeProperty>
  <owl:DatatypeProperty rdf:about="http://example.org/onto/prop/google_network_security_authz_policy_prefix">
    <rdfs:label>prefix</rdfs:label>
    <rdfs:comment>The input string must have the prefix specified here. Note: empty prefix is not allowed, please use regex instead.
Examples:
* abc matches the value abc.xyz</rdfs:comment>
    <rdfs:domain rdf:resource="http://example.org/onto/class/google_network_security_authz_policy"/>
    <rdfs:range rdf:resource="http://www.w3.org/2001/XMLSchema#string"/>
  </owl:DatatypeProperty>
  <owl:DatatypeProperty rdf:about="http://example.org/onto/prop/google_network_security_authz_policy_suffix">
    <rdfs:label>suffix</rdfs:label>
    <rdfs:comment>The input string must have the suffix specified here. Note: empty prefix is not allowed, please use regex instead.
Examples:
* abc matches the value xyz.abc</rdfs:comment>
    <rdfs:domain rdf:resource="http://example.org/onto/class/google_network_security_authz_policy"/>
    <rdfs:range rdf:resource="http://www.w3.org/2001/XMLSchema#string"/>
  </owl:DatatypeProperty>
  <owl:DatatypeProperty rdf:about="http://example.org/onto/prop/google_network_security_authz_policy_load_balancing_scheme">
    <rdfs:label>load_balancing_scheme</rdfs:label>
    <rdfs:comment>All gateways and forwarding rules referenced by this policy and extensions must share the same load balancing scheme.
For more information, refer to [Backend services overview](https://cloud.google.com/load-balancing/docs/backend-service). Possible values: ["INTERNAL_MANAGED", "EXTERNAL_MANAGED", "INTERNAL_SELF_MANAGED"]</rdfs:comment>
    <rdfs:domain rdf:resource="http://example.org/onto/class/google_network_security_authz_policy"/>
    <rdfs:range rdf:resource="http://www.w3.org/2001/XMLSchema#string"/>
  </owl:DatatypeProperty>
  <owl:DatatypeProperty rdf:about="http://example.org/onto/prop/google_network_security_authz_policy_resources">
    <rdfs:label>resources</rdfs:label>
    <rdfs:comment>A list of references to the Forwarding Rules on which this policy will be applied.</rdfs:comment>
    <rdfs:domain rdf:resource="http://example.org/onto/class/google_network_security_authz_policy"/>
    <rdfs:range rdf:resource="http://www.w3.org/2001/XMLSchema#string"/>
  </owl:DatatypeProperty>
  <owl:DatatypeProperty rdf:about="http://example.org/onto/prop/google_network_security_authz_policy_create">
    <rdfs:label>create</rdfs:label>
    <rdfs:domain rdf:resource="http://example.org/onto/class/google_network_security_authz_policy"/>
    <rdfs:range rdf:resource="http://www.w3.org/2001/XMLSchema#string"/>
  </owl:DatatypeProperty>
  <owl:DatatypeProperty rdf:about="http://example.org/onto/prop/google_network_security_authz_policy_delete">
    <rdfs:label>delete</rdfs:label>
    <rdfs:domain rdf:resource="http://example.org/onto/class/google_network_security_authz_policy"/>
    <rdfs:range rdf:resource="http://www.w3.org/2001/XMLSchema#string"/>
  </owl:DatatypeProperty>
  <owl:DatatypeProperty rdf:about="http://example.org/onto/prop/google_network_security_authz_policy_update">
    <rdfs:label>update</rdfs:label>
    <rdfs:domain rdf:resource="http://example.org/onto/class/google_network_security_authz_policy"/>
    <rdfs:range rdf:resource="http://www.w3.org/2001/XMLSchema#string"/>
  </owl:DatatypeProperty>
</rdf:RDF>
