<?xml version="1.0" encoding="UTF-8"?>
<rdf:RDF
  xmlns:rdf="http://www.w3.org/1999/02/22-rdf-syntax-ns#"
  xmlns:rdfs="http://www.w3.org/2000/01/rdf-schema#"
  xmlns:owl="http://www.w3.org/2002/07/owl#"
  xmlns:xsd="http://www.w3.org/2001/XMLSchema#"
  xml:base="http://example.org/onto/">
  <owl:Class rdf:about="http://example.org/onto/class/google_firebase_app_check_recaptcha_v3_config">
    <rdfs:label>google_firebase_app_check_recaptcha_v3_config</rdfs:label>
    <rdfs:comment>#
#     ***     AUTO GENERATED CODE    ***    Type: MMv1     ***
#
# ----------------------------------------------------------------------------
#
#     This code is generated by Magic Modules using the following:
#
#     Configuration: https:#github.com/GoogleCloudPlatform/magic-modules/tree/main/mmv1/products/firebaseappcheck/RecaptchaV3Config.yaml
#     Template:      https:#github.com/GoogleCloudPlatform/magic-modules/tree/main/mmv1/templates/terraform/resource.html.markdown.tmpl
#
#     DO NOT EDIT this file directly. Any changes made to this file will be
#     overwritten during the next generation cycle.
#
# ----------------------------------------------------------------------------
subcategory: "Firebase App Check"
description: |-
  An app's reCAPTCHA V3 configuration object.
---</rdfs:comment>
  </owl:Class>
  <owl:DatatypeProperty rdf:about="http://example.org/onto/prop/google_firebase_app_check_recaptcha_v3_config_app_id">
    <rdfs:label>app_id</rdfs:label>
    <rdfs:comment>The ID of an
[Web App](https://firebase.google.com/docs/reference/firebase-management/rest/v1beta1/projects.webApps#WebApp.FIELDS.app_id).</rdfs:comment>
    <rdfs:domain rdf:resource="http://example.org/onto/class/google_firebase_app_check_recaptcha_v3_config"/>
    <rdfs:range rdf:resource="http://www.w3.org/2001/XMLSchema#string"/>
  </owl:DatatypeProperty>
  <owl:DatatypeProperty rdf:about="http://example.org/onto/prop/google_firebase_app_check_recaptcha_v3_config_id">
    <rdfs:label>id</rdfs:label>
    <rdfs:domain rdf:resource="http://example.org/onto/class/google_firebase_app_check_recaptcha_v3_config"/>
    <rdfs:range rdf:resource="http://www.w3.org/2001/XMLSchema#string"/>
  </owl:DatatypeProperty>
  <owl:DatatypeProperty rdf:about="http://example.org/onto/prop/google_firebase_app_check_recaptcha_v3_config_name">
    <rdfs:label>name</rdfs:label>
    <rdfs:comment>The relative resource name of the reCAPTCHA V3 configuration object</rdfs:comment>
    <rdfs:domain rdf:resource="http://example.org/onto/class/google_firebase_app_check_recaptcha_v3_config"/>
    <rdfs:range rdf:resource="http://www.w3.org/2001/XMLSchema#string"/>
  </owl:DatatypeProperty>
  <owl:DatatypeProperty rdf:about="http://example.org/onto/prop/google_firebase_app_check_recaptcha_v3_config_project">
    <rdfs:label>project</rdfs:label>
    <rdfs:domain rdf:resource="http://example.org/onto/class/google_firebase_app_check_recaptcha_v3_config"/>
    <rdfs:range rdf:resource="http://www.w3.org/2001/XMLSchema#string"/>
  </owl:DatatypeProperty>
  <owl:DatatypeProperty rdf:about="http://example.org/onto/prop/google_firebase_app_check_recaptcha_v3_config_site_secret">
    <rdfs:label>site_secret</rdfs:label>
    <rdfs:comment>The site secret used to identify your service for reCAPTCHA v3 verification.
For security reasons, this field will never be populated in any response.</rdfs:comment>
    <rdfs:domain rdf:resource="http://example.org/onto/class/google_firebase_app_check_recaptcha_v3_config"/>
    <rdfs:range rdf:resource="http://www.w3.org/2001/XMLSchema#string"/>
  </owl:DatatypeProperty>
  <owl:DatatypeProperty rdf:about="http://example.org/onto/prop/google_firebase_app_check_recaptcha_v3_config_site_secret_set">
    <rdfs:label>site_secret_set</rdfs:label>
    <rdfs:comment>Whether the siteSecret was previously set. Since we will never return the siteSecret field, this field is the only way to find out whether it was previously set.</rdfs:comment>
    <rdfs:domain rdf:resource="http://example.org/onto/class/google_firebase_app_check_recaptcha_v3_config"/>
    <rdfs:range rdf:resource="http://www.w3.org/2001/XMLSchema#string"/>
  </owl:DatatypeProperty>
  <owl:DatatypeProperty rdf:about="http://example.org/onto/prop/google_firebase_app_check_recaptcha_v3_config_token_ttl">
    <rdfs:label>token_ttl</rdfs:label>
    <rdfs:comment>Specifies the duration for which App Check tokens exchanged from reCAPTCHA V3 artifacts will be valid.
If unset, a default value of 1 hour is assumed. Must be between 30 minutes and 7 days, inclusive.

A duration in seconds with up to nine fractional digits, ending with 's'. Example: "3.5s".</rdfs:comment>
    <rdfs:domain rdf:resource="http://example.org/onto/class/google_firebase_app_check_recaptcha_v3_config"/>
    <rdfs:range rdf:resource="http://www.w3.org/2001/XMLSchema#string"/>
  </owl:DatatypeProperty>
  <owl:DatatypeProperty rdf:about="http://example.org/onto/prop/google_firebase_app_check_recaptcha_v3_config_create">
    <rdfs:label>create</rdfs:label>
    <rdfs:domain rdf:resource="http://example.org/onto/class/google_firebase_app_check_recaptcha_v3_config"/>
    <rdfs:range rdf:resource="http://www.w3.org/2001/XMLSchema#string"/>
  </owl:DatatypeProperty>
  <owl:DatatypeProperty rdf:about="http://example.org/onto/prop/google_firebase_app_check_recaptcha_v3_config_delete">
    <rdfs:label>delete</rdfs:label>
    <rdfs:domain rdf:resource="http://example.org/onto/class/google_firebase_app_check_recaptcha_v3_config"/>
    <rdfs:range rdf:resource="http://www.w3.org/2001/XMLSchema#string"/>
  </owl:DatatypeProperty>
  <owl:DatatypeProperty rdf:about="http://example.org/onto/prop/google_firebase_app_check_recaptcha_v3_config_update">
    <rdfs:label>update</rdfs:label>
    <rdfs:domain rdf:resource="http://example.org/onto/class/google_firebase_app_check_recaptcha_v3_config"/>
    <rdfs:range rdf:resource="http://www.w3.org/2001/XMLSchema#string"/>
  </owl:DatatypeProperty>
</rdf:RDF>
