<?xml version="1.0" encoding="UTF-8"?>
<rdf:RDF
  xmlns:rdf="http://www.w3.org/1999/02/22-rdf-syntax-ns#"
  xmlns:rdfs="http://www.w3.org/2000/01/rdf-schema#"
  xmlns:owl="http://www.w3.org/2002/07/owl#"
  xmlns:xsd="http://www.w3.org/2001/XMLSchema#"
  xml:base="http://example.org/onto/">
  <owl:Class rdf:about="http://example.org/onto/class/google_looker_instance">
    <rdfs:label>google_looker_instance</rdfs:label>
    <rdfs:comment>#
#     ***     AUTO GENERATED CODE    ***    Type: MMv1     ***
#
# ----------------------------------------------------------------------------
#
#     This code is generated by Magic Modules using the following:
#
#     Configuration: https:#github.com/GoogleCloudPlatform/magic-modules/tree/main/mmv1/products/looker/Instance.yaml
#     Template:      https:#github.com/GoogleCloudPlatform/magic-modules/tree/main/mmv1/templates/terraform/resource.html.markdown.tmpl
#
#     DO NOT EDIT this file directly. Any changes made to this file will be
#     overwritten during the next generation cycle.
#
# ----------------------------------------------------------------------------
subcategory: "Looker (Google Cloud core)"
description: |-
  A Google Cloud Looker instance.
---</rdfs:comment>
  </owl:Class>
  <owl:DatatypeProperty rdf:about="http://example.org/onto/prop/google_looker_instance_consumer_network">
    <rdfs:label>consumer_network</rdfs:label>
    <rdfs:comment>Network name in the consumer project in the format of: projects/{project}/global/networks/{network}
Note that the consumer network may be in a different GCP project than the consumer
project that is hosting the Looker Instance.</rdfs:comment>
    <rdfs:domain rdf:resource="http://example.org/onto/class/google_looker_instance"/>
    <rdfs:range rdf:resource="http://www.w3.org/2001/XMLSchema#string"/>
  </owl:DatatypeProperty>
  <owl:DatatypeProperty rdf:about="http://example.org/onto/prop/google_looker_instance_create_time">
    <rdfs:label>create_time</rdfs:label>
    <rdfs:comment>The time the instance was created in RFC3339 UTC "Zulu" format,
accurate to nanoseconds.</rdfs:comment>
    <rdfs:domain rdf:resource="http://example.org/onto/class/google_looker_instance"/>
    <rdfs:range rdf:resource="http://www.w3.org/2001/XMLSchema#string"/>
  </owl:DatatypeProperty>
  <owl:DatatypeProperty rdf:about="http://example.org/onto/prop/google_looker_instance_deletion_policy">
    <rdfs:label>deletion_policy</rdfs:label>
    <rdfs:comment>Policy to determine if the cluster should be deleted forcefully.
If setting deletion_policy = "FORCE", the Looker instance will be deleted regardless
of its nested resources. If set to "DEFAULT", Looker instances that still have
nested resources will return an error. Possible values: DEFAULT, FORCE</rdfs:comment>
    <rdfs:domain rdf:resource="http://example.org/onto/class/google_looker_instance"/>
    <rdfs:range rdf:resource="http://www.w3.org/2001/XMLSchema#string"/>
  </owl:DatatypeProperty>
  <owl:DatatypeProperty rdf:about="http://example.org/onto/prop/google_looker_instance_egress_public_ip">
    <rdfs:label>egress_public_ip</rdfs:label>
    <rdfs:comment>Public Egress IP (IPv4).</rdfs:comment>
    <rdfs:domain rdf:resource="http://example.org/onto/class/google_looker_instance"/>
    <rdfs:range rdf:resource="http://www.w3.org/2001/XMLSchema#string"/>
  </owl:DatatypeProperty>
  <owl:DatatypeProperty rdf:about="http://example.org/onto/prop/google_looker_instance_fips_enabled">
    <rdfs:label>fips_enabled</rdfs:label>
    <rdfs:comment>FIPS 140-2 Encryption enablement for Looker (Google Cloud Core).</rdfs:comment>
    <rdfs:domain rdf:resource="http://example.org/onto/class/google_looker_instance"/>
    <rdfs:range rdf:resource="http://www.w3.org/2001/XMLSchema#string"/>
  </owl:DatatypeProperty>
  <owl:DatatypeProperty rdf:about="http://example.org/onto/prop/google_looker_instance_gemini_enabled">
    <rdfs:label>gemini_enabled</rdfs:label>
    <rdfs:comment>Gemini enablement for Looker (Google Cloud Core).</rdfs:comment>
    <rdfs:domain rdf:resource="http://example.org/onto/class/google_looker_instance"/>
    <rdfs:range rdf:resource="http://www.w3.org/2001/XMLSchema#string"/>
  </owl:DatatypeProperty>
  <owl:DatatypeProperty rdf:about="http://example.org/onto/prop/google_looker_instance_id">
    <rdfs:label>id</rdfs:label>
    <rdfs:domain rdf:resource="http://example.org/onto/class/google_looker_instance"/>
    <rdfs:range rdf:resource="http://www.w3.org/2001/XMLSchema#string"/>
  </owl:DatatypeProperty>
  <owl:DatatypeProperty rdf:about="http://example.org/onto/prop/google_looker_instance_ingress_private_ip">
    <rdfs:label>ingress_private_ip</rdfs:label>
    <rdfs:comment>Private Ingress IP (IPv4).</rdfs:comment>
    <rdfs:domain rdf:resource="http://example.org/onto/class/google_looker_instance"/>
    <rdfs:range rdf:resource="http://www.w3.org/2001/XMLSchema#string"/>
  </owl:DatatypeProperty>
  <owl:DatatypeProperty rdf:about="http://example.org/onto/prop/google_looker_instance_ingress_public_ip">
    <rdfs:label>ingress_public_ip</rdfs:label>
    <rdfs:comment>Public Ingress IP (IPv4).</rdfs:comment>
    <rdfs:domain rdf:resource="http://example.org/onto/class/google_looker_instance"/>
    <rdfs:range rdf:resource="http://www.w3.org/2001/XMLSchema#string"/>
  </owl:DatatypeProperty>
  <owl:DatatypeProperty rdf:about="http://example.org/onto/prop/google_looker_instance_looker_uri">
    <rdfs:label>looker_uri</rdfs:label>
    <rdfs:comment>Looker instance URI which can be used to access the Looker Instance UI.</rdfs:comment>
    <rdfs:domain rdf:resource="http://example.org/onto/class/google_looker_instance"/>
    <rdfs:range rdf:resource="http://www.w3.org/2001/XMLSchema#string"/>
  </owl:DatatypeProperty>
  <owl:DatatypeProperty rdf:about="http://example.org/onto/prop/google_looker_instance_looker_version">
    <rdfs:label>looker_version</rdfs:label>
    <rdfs:comment>The Looker version that the instance is using.</rdfs:comment>
    <rdfs:domain rdf:resource="http://example.org/onto/class/google_looker_instance"/>
    <rdfs:range rdf:resource="http://www.w3.org/2001/XMLSchema#string"/>
  </owl:DatatypeProperty>
  <owl:DatatypeProperty rdf:about="http://example.org/onto/prop/google_looker_instance_name">
    <rdfs:label>name</rdfs:label>
    <rdfs:comment>The ID of the instance or a fully qualified identifier for the instance.</rdfs:comment>
    <rdfs:domain rdf:resource="http://example.org/onto/class/google_looker_instance"/>
    <rdfs:range rdf:resource="http://www.w3.org/2001/XMLSchema#string"/>
  </owl:DatatypeProperty>
  <owl:DatatypeProperty rdf:about="http://example.org/onto/prop/google_looker_instance_platform_edition">
    <rdfs:label>platform_edition</rdfs:label>
    <rdfs:comment>Platform editions for a Looker instance. Each edition maps to a set of instance features, like its size. Must be one of these values:
- LOOKER_CORE_TRIAL: trial instance (Currently Unavailable)
- LOOKER_CORE_STANDARD: pay as you go standard instance (Currently Unavailable)
- LOOKER_CORE_STANDARD_ANNUAL: subscription standard instance
- LOOKER_CORE_ENTERPRISE_ANNUAL: subscription enterprise instance
- LOOKER_CORE_EMBED_ANNUAL: subscription embed instance
- LOOKER_CORE_NONPROD_STANDARD_ANNUAL: nonprod subscription standard instance
- LOOKER_CORE_NONPROD_ENTERPRISE_ANNUAL: nonprod subscription enterprise instance
- LOOKER_CORE_NONPROD_EMBED_ANNUAL: nonprod subscription embed instance
- LOOKER_CORE_TRIAL_STANDARD: A standard trial edition of Looker (Google Cloud core) product.
- LOOKER_CORE_TRIAL_ENTERPRISE: An enterprise trial edition of Looker (Google Cloud core) product.
- LOOKER_CORE_TRIAL_EMBED: An embed trial edition of Looker (Google Cloud core) product. Default value: "LOOKER_CORE_TRIAL" Possible values: ["LOOKER_CORE_TRIAL", "LOOKER_CORE_STANDARD", "LOOKER_CORE_STANDARD_ANNUAL", "LOOKER_CORE_ENTERPRISE_ANNUAL", "LOOKER_CORE_EMBED_ANNUAL", "LOOKER_CORE_NONPROD_STANDARD_ANNUAL", "LOOKER_CORE_NONPROD_ENTERPRISE_ANNUAL", "LOOKER_CORE_NONPROD_EMBED_ANNUAL", "LOOKER_CORE_TRIAL_STANDARD", "LOOKER_CORE_TRIAL_ENTERPRISE", "LOOKER_CORE_TRIAL_EMBED"]</rdfs:comment>
    <rdfs:domain rdf:resource="http://example.org/onto/class/google_looker_instance"/>
    <rdfs:range rdf:resource="http://www.w3.org/2001/XMLSchema#string"/>
  </owl:DatatypeProperty>
  <owl:DatatypeProperty rdf:about="http://example.org/onto/prop/google_looker_instance_private_ip_enabled">
    <rdfs:label>private_ip_enabled</rdfs:label>
    <rdfs:comment>Whether private IP is enabled on the Looker instance.</rdfs:comment>
    <rdfs:domain rdf:resource="http://example.org/onto/class/google_looker_instance"/>
    <rdfs:range rdf:resource="http://www.w3.org/2001/XMLSchema#string"/>
  </owl:DatatypeProperty>
  <owl:DatatypeProperty rdf:about="http://example.org/onto/prop/google_looker_instance_project">
    <rdfs:label>project</rdfs:label>
    <rdfs:domain rdf:resource="http://example.org/onto/class/google_looker_instance"/>
    <rdfs:range rdf:resource="http://www.w3.org/2001/XMLSchema#string"/>
  </owl:DatatypeProperty>
  <owl:DatatypeProperty rdf:about="http://example.org/onto/prop/google_looker_instance_psc_enabled">
    <rdfs:label>psc_enabled</rdfs:label>
    <rdfs:comment>Whether Public Service Connect (PSC) is enabled on the Looker instance</rdfs:comment>
    <rdfs:domain rdf:resource="http://example.org/onto/class/google_looker_instance"/>
    <rdfs:range rdf:resource="http://www.w3.org/2001/XMLSchema#string"/>
  </owl:DatatypeProperty>
  <owl:DatatypeProperty rdf:about="http://example.org/onto/prop/google_looker_instance_public_ip_enabled">
    <rdfs:label>public_ip_enabled</rdfs:label>
    <rdfs:comment>Whether public IP is enabled on the Looker instance.</rdfs:comment>
    <rdfs:domain rdf:resource="http://example.org/onto/class/google_looker_instance"/>
    <rdfs:range rdf:resource="http://www.w3.org/2001/XMLSchema#string"/>
  </owl:DatatypeProperty>
  <owl:DatatypeProperty rdf:about="http://example.org/onto/prop/google_looker_instance_region">
    <rdfs:label>region</rdfs:label>
    <rdfs:comment>The name of the Looker region of the instance.</rdfs:comment>
    <rdfs:domain rdf:resource="http://example.org/onto/class/google_looker_instance"/>
    <rdfs:range rdf:resource="http://www.w3.org/2001/XMLSchema#string"/>
  </owl:DatatypeProperty>
  <owl:DatatypeProperty rdf:about="http://example.org/onto/prop/google_looker_instance_reserved_range">
    <rdfs:label>reserved_range</rdfs:label>
    <rdfs:comment>Name of a reserved IP address range within the consumer network, to be used for
private service access connection. User may or may not specify this in a request.</rdfs:comment>
    <rdfs:domain rdf:resource="http://example.org/onto/class/google_looker_instance"/>
    <rdfs:range rdf:resource="http://www.w3.org/2001/XMLSchema#string"/>
  </owl:DatatypeProperty>
  <owl:DatatypeProperty rdf:about="http://example.org/onto/prop/google_looker_instance_update_time">
    <rdfs:label>update_time</rdfs:label>
    <rdfs:comment>The time the instance was updated in RFC3339 UTC "Zulu" format,
accurate to nanoseconds.</rdfs:comment>
    <rdfs:domain rdf:resource="http://example.org/onto/class/google_looker_instance"/>
    <rdfs:range rdf:resource="http://www.w3.org/2001/XMLSchema#string"/>
  </owl:DatatypeProperty>
  <owl:DatatypeProperty rdf:about="http://example.org/onto/prop/google_looker_instance_allowed_email_domains">
    <rdfs:label>allowed_email_domains</rdfs:label>
    <rdfs:comment>Email domain allowlist for the instance.

Define the email domains to which your users can deliver Looker (Google Cloud core) content.
Updating this list will restart the instance. Updating the allowed email domains from terraform
means the value provided will be considered as the entire list and not an amendment to the
existing list of allowed email domains.</rdfs:comment>
    <rdfs:domain rdf:resource="http://example.org/onto/class/google_looker_instance"/>
    <rdfs:range rdf:resource="http://www.w3.org/2001/XMLSchema#string"/>
  </owl:DatatypeProperty>
  <owl:DatatypeProperty rdf:about="http://example.org/onto/prop/google_looker_instance_domain">
    <rdfs:label>domain</rdfs:label>
    <rdfs:comment>Domain name</rdfs:comment>
    <rdfs:domain rdf:resource="http://example.org/onto/class/google_looker_instance"/>
    <rdfs:range rdf:resource="http://www.w3.org/2001/XMLSchema#string"/>
  </owl:DatatypeProperty>
  <owl:DatatypeProperty rdf:about="http://example.org/onto/prop/google_looker_instance_state">
    <rdfs:label>state</rdfs:label>
    <rdfs:comment>Status of the custom domain.</rdfs:comment>
    <rdfs:domain rdf:resource="http://example.org/onto/class/google_looker_instance"/>
    <rdfs:range rdf:resource="http://www.w3.org/2001/XMLSchema#string"/>
  </owl:DatatypeProperty>
  <owl:DatatypeProperty rdf:about="http://example.org/onto/prop/google_looker_instance_day">
    <rdfs:label>day</rdfs:label>
    <rdfs:comment>Day of a month. Must be from 1 to 31 and valid for the year and month, or 0
to specify a year by itself or a year and month where the day isn't significant.</rdfs:comment>
    <rdfs:domain rdf:resource="http://example.org/onto/class/google_looker_instance"/>
    <rdfs:range rdf:resource="http://www.w3.org/2001/XMLSchema#string"/>
  </owl:DatatypeProperty>
  <owl:DatatypeProperty rdf:about="http://example.org/onto/prop/google_looker_instance_month">
    <rdfs:label>month</rdfs:label>
    <rdfs:comment>Month of a year. Must be from 1 to 12, or 0 to specify a year without a
month and day.</rdfs:comment>
    <rdfs:domain rdf:resource="http://example.org/onto/class/google_looker_instance"/>
    <rdfs:range rdf:resource="http://www.w3.org/2001/XMLSchema#string"/>
  </owl:DatatypeProperty>
  <owl:DatatypeProperty rdf:about="http://example.org/onto/prop/google_looker_instance_year">
    <rdfs:label>year</rdfs:label>
    <rdfs:comment>Year of the date. Must be from 1 to 9999, or 0 to specify a date without
a year.</rdfs:comment>
    <rdfs:domain rdf:resource="http://example.org/onto/class/google_looker_instance"/>
    <rdfs:range rdf:resource="http://www.w3.org/2001/XMLSchema#string"/>
  </owl:DatatypeProperty>
  <owl:DatatypeProperty rdf:about="http://example.org/onto/prop/google_looker_instance_day">
    <rdfs:label>day</rdfs:label>
    <rdfs:comment>Day of a month. Must be from 1 to 31 and valid for the year and month, or 0
to specify a year by itself or a year and month where the day isn't significant.</rdfs:comment>
    <rdfs:domain rdf:resource="http://example.org/onto/class/google_looker_instance"/>
    <rdfs:range rdf:resource="http://www.w3.org/2001/XMLSchema#string"/>
  </owl:DatatypeProperty>
  <owl:DatatypeProperty rdf:about="http://example.org/onto/prop/google_looker_instance_month">
    <rdfs:label>month</rdfs:label>
    <rdfs:comment>Month of a year. Must be from 1 to 12, or 0 to specify a year without a
month and day.</rdfs:comment>
    <rdfs:domain rdf:resource="http://example.org/onto/class/google_looker_instance"/>
    <rdfs:range rdf:resource="http://www.w3.org/2001/XMLSchema#string"/>
  </owl:DatatypeProperty>
  <owl:DatatypeProperty rdf:about="http://example.org/onto/prop/google_looker_instance_year">
    <rdfs:label>year</rdfs:label>
    <rdfs:comment>Year of the date. Must be from 1 to 9999, or 0 to specify a date without
a year.</rdfs:comment>
    <rdfs:domain rdf:resource="http://example.org/onto/class/google_looker_instance"/>
    <rdfs:range rdf:resource="http://www.w3.org/2001/XMLSchema#string"/>
  </owl:DatatypeProperty>
  <owl:DatatypeProperty rdf:about="http://example.org/onto/prop/google_looker_instance_hours">
    <rdfs:label>hours</rdfs:label>
    <rdfs:comment>Hours of day in 24 hour format. Should be from 0 to 23.</rdfs:comment>
    <rdfs:domain rdf:resource="http://example.org/onto/class/google_looker_instance"/>
    <rdfs:range rdf:resource="http://www.w3.org/2001/XMLSchema#string"/>
  </owl:DatatypeProperty>
  <owl:DatatypeProperty rdf:about="http://example.org/onto/prop/google_looker_instance_minutes">
    <rdfs:label>minutes</rdfs:label>
    <rdfs:comment>Minutes of hour of day. Must be from 0 to 59.</rdfs:comment>
    <rdfs:domain rdf:resource="http://example.org/onto/class/google_looker_instance"/>
    <rdfs:range rdf:resource="http://www.w3.org/2001/XMLSchema#string"/>
  </owl:DatatypeProperty>
  <owl:DatatypeProperty rdf:about="http://example.org/onto/prop/google_looker_instance_nanos">
    <rdfs:label>nanos</rdfs:label>
    <rdfs:comment>Fractions of seconds in nanoseconds. Must be from 0 to 999,999,999.</rdfs:comment>
    <rdfs:domain rdf:resource="http://example.org/onto/class/google_looker_instance"/>
    <rdfs:range rdf:resource="http://www.w3.org/2001/XMLSchema#string"/>
  </owl:DatatypeProperty>
  <owl:DatatypeProperty rdf:about="http://example.org/onto/prop/google_looker_instance_seconds">
    <rdfs:label>seconds</rdfs:label>
    <rdfs:comment>Seconds of minutes of the time. Must normally be from 0 to 59.</rdfs:comment>
    <rdfs:domain rdf:resource="http://example.org/onto/class/google_looker_instance"/>
    <rdfs:range rdf:resource="http://www.w3.org/2001/XMLSchema#string"/>
  </owl:DatatypeProperty>
  <owl:DatatypeProperty rdf:about="http://example.org/onto/prop/google_looker_instance_kms_key_name">
    <rdfs:label>kms_key_name</rdfs:label>
    <rdfs:comment>Name of the customer managed encryption key (CMEK) in KMS.</rdfs:comment>
    <rdfs:domain rdf:resource="http://example.org/onto/class/google_looker_instance"/>
    <rdfs:range rdf:resource="http://www.w3.org/2001/XMLSchema#string"/>
  </owl:DatatypeProperty>
  <owl:DatatypeProperty rdf:about="http://example.org/onto/prop/google_looker_instance_kms_key_name_version">
    <rdfs:label>kms_key_name_version</rdfs:label>
    <rdfs:comment>Full name and version of the CMEK key currently in use to encrypt Looker data.</rdfs:comment>
    <rdfs:domain rdf:resource="http://example.org/onto/class/google_looker_instance"/>
    <rdfs:range rdf:resource="http://www.w3.org/2001/XMLSchema#string"/>
  </owl:DatatypeProperty>
  <owl:DatatypeProperty rdf:about="http://example.org/onto/prop/google_looker_instance_kms_key_state">
    <rdfs:label>kms_key_state</rdfs:label>
    <rdfs:comment>Status of the customer managed encryption key (CMEK) in KMS.</rdfs:comment>
    <rdfs:domain rdf:resource="http://example.org/onto/class/google_looker_instance"/>
    <rdfs:range rdf:resource="http://www.w3.org/2001/XMLSchema#string"/>
  </owl:DatatypeProperty>
  <owl:DatatypeProperty rdf:about="http://example.org/onto/prop/google_looker_instance_day_of_week">
    <rdfs:label>day_of_week</rdfs:label>
    <rdfs:comment>Required. Day of the week for this MaintenanceWindow (in UTC).

- MONDAY: Monday
- TUESDAY: Tuesday
- WEDNESDAY: Wednesday
- THURSDAY: Thursday
- FRIDAY: Friday
- SATURDAY: Saturday
- SUNDAY: Sunday Possible values: ["MONDAY", "TUESDAY", "WEDNESDAY", "THURSDAY", "FRIDAY", "SATURDAY", "SUNDAY"]</rdfs:comment>
    <rdfs:domain rdf:resource="http://example.org/onto/class/google_looker_instance"/>
    <rdfs:range rdf:resource="http://www.w3.org/2001/XMLSchema#string"/>
  </owl:DatatypeProperty>
  <owl:DatatypeProperty rdf:about="http://example.org/onto/prop/google_looker_instance_hours">
    <rdfs:label>hours</rdfs:label>
    <rdfs:comment>Hours of day in 24 hour format. Should be from 0 to 23.</rdfs:comment>
    <rdfs:domain rdf:resource="http://example.org/onto/class/google_looker_instance"/>
    <rdfs:range rdf:resource="http://www.w3.org/2001/XMLSchema#string"/>
  </owl:DatatypeProperty>
  <owl:DatatypeProperty rdf:about="http://example.org/onto/prop/google_looker_instance_minutes">
    <rdfs:label>minutes</rdfs:label>
    <rdfs:comment>Minutes of hour of day. Must be from 0 to 59.</rdfs:comment>
    <rdfs:domain rdf:resource="http://example.org/onto/class/google_looker_instance"/>
    <rdfs:range rdf:resource="http://www.w3.org/2001/XMLSchema#string"/>
  </owl:DatatypeProperty>
  <owl:DatatypeProperty rdf:about="http://example.org/onto/prop/google_looker_instance_nanos">
    <rdfs:label>nanos</rdfs:label>
    <rdfs:comment>Fractions of seconds in nanoseconds. Must be from 0 to 999,999,999.</rdfs:comment>
    <rdfs:domain rdf:resource="http://example.org/onto/class/google_looker_instance"/>
    <rdfs:range rdf:resource="http://www.w3.org/2001/XMLSchema#string"/>
  </owl:DatatypeProperty>
  <owl:DatatypeProperty rdf:about="http://example.org/onto/prop/google_looker_instance_seconds">
    <rdfs:label>seconds</rdfs:label>
    <rdfs:comment>Seconds of minutes of the time. Must normally be from 0 to 59.</rdfs:comment>
    <rdfs:domain rdf:resource="http://example.org/onto/class/google_looker_instance"/>
    <rdfs:range rdf:resource="http://www.w3.org/2001/XMLSchema#string"/>
  </owl:DatatypeProperty>
  <owl:DatatypeProperty rdf:about="http://example.org/onto/prop/google_looker_instance_client_id">
    <rdfs:label>client_id</rdfs:label>
    <rdfs:comment>The client ID for the Oauth config.</rdfs:comment>
    <rdfs:domain rdf:resource="http://example.org/onto/class/google_looker_instance"/>
    <rdfs:range rdf:resource="http://www.w3.org/2001/XMLSchema#string"/>
  </owl:DatatypeProperty>
  <owl:DatatypeProperty rdf:about="http://example.org/onto/prop/google_looker_instance_client_secret">
    <rdfs:label>client_secret</rdfs:label>
    <rdfs:comment>The client secret for the Oauth config.</rdfs:comment>
    <rdfs:domain rdf:resource="http://example.org/onto/class/google_looker_instance"/>
    <rdfs:range rdf:resource="http://www.w3.org/2001/XMLSchema#string"/>
  </owl:DatatypeProperty>
  <owl:DatatypeProperty rdf:about="http://example.org/onto/prop/google_looker_instance_allowed_vpcs">
    <rdfs:label>allowed_vpcs</rdfs:label>
    <rdfs:comment>List of VPCs that are allowed ingress into the Looker instance.</rdfs:comment>
    <rdfs:domain rdf:resource="http://example.org/onto/class/google_looker_instance"/>
    <rdfs:range rdf:resource="http://www.w3.org/2001/XMLSchema#string"/>
  </owl:DatatypeProperty>
  <owl:DatatypeProperty rdf:about="http://example.org/onto/prop/google_looker_instance_looker_service_attachment_uri">
    <rdfs:label>looker_service_attachment_uri</rdfs:label>
    <rdfs:comment>URI of the Looker service attachment.</rdfs:comment>
    <rdfs:domain rdf:resource="http://example.org/onto/class/google_looker_instance"/>
    <rdfs:range rdf:resource="http://www.w3.org/2001/XMLSchema#string"/>
  </owl:DatatypeProperty>
  <owl:DatatypeProperty rdf:about="http://example.org/onto/prop/google_looker_instance_connection_status">
    <rdfs:label>connection_status</rdfs:label>
    <rdfs:comment>Status of the service attachment connection.</rdfs:comment>
    <rdfs:domain rdf:resource="http://example.org/onto/class/google_looker_instance"/>
    <rdfs:range rdf:resource="http://www.w3.org/2001/XMLSchema#string"/>
  </owl:DatatypeProperty>
  <owl:DatatypeProperty rdf:about="http://example.org/onto/prop/google_looker_instance_local_fqdn">
    <rdfs:label>local_fqdn</rdfs:label>
    <rdfs:comment>Fully qualified domain name that will be used in the private DNS record created for the service attachment.</rdfs:comment>
    <rdfs:domain rdf:resource="http://example.org/onto/class/google_looker_instance"/>
    <rdfs:range rdf:resource="http://www.w3.org/2001/XMLSchema#string"/>
  </owl:DatatypeProperty>
  <owl:DatatypeProperty rdf:about="http://example.org/onto/prop/google_looker_instance_target_service_attachment_uri">
    <rdfs:label>target_service_attachment_uri</rdfs:label>
    <rdfs:comment>URI of the service attachment to connect to.</rdfs:comment>
    <rdfs:domain rdf:resource="http://example.org/onto/class/google_looker_instance"/>
    <rdfs:range rdf:resource="http://www.w3.org/2001/XMLSchema#string"/>
  </owl:DatatypeProperty>
  <owl:DatatypeProperty rdf:about="http://example.org/onto/prop/google_looker_instance_create">
    <rdfs:label>create</rdfs:label>
    <rdfs:domain rdf:resource="http://example.org/onto/class/google_looker_instance"/>
    <rdfs:range rdf:resource="http://www.w3.org/2001/XMLSchema#string"/>
  </owl:DatatypeProperty>
  <owl:DatatypeProperty rdf:about="http://example.org/onto/prop/google_looker_instance_delete">
    <rdfs:label>delete</rdfs:label>
    <rdfs:domain rdf:resource="http://example.org/onto/class/google_looker_instance"/>
    <rdfs:range rdf:resource="http://www.w3.org/2001/XMLSchema#string"/>
  </owl:DatatypeProperty>
  <owl:DatatypeProperty rdf:about="http://example.org/onto/prop/google_looker_instance_update">
    <rdfs:label>update</rdfs:label>
    <rdfs:domain rdf:resource="http://example.org/onto/class/google_looker_instance"/>
    <rdfs:range rdf:resource="http://www.w3.org/2001/XMLSchema#string"/>
  </owl:DatatypeProperty>
  <owl:DatatypeProperty rdf:about="http://example.org/onto/prop/google_looker_instance_additional_developer_user_count">
    <rdfs:label>additional_developer_user_count</rdfs:label>
    <rdfs:comment>Number of additional Developer Users to allocate to the Looker Instance.</rdfs:comment>
    <rdfs:domain rdf:resource="http://example.org/onto/class/google_looker_instance"/>
    <rdfs:range rdf:resource="http://www.w3.org/2001/XMLSchema#string"/>
  </owl:DatatypeProperty>
  <owl:DatatypeProperty rdf:about="http://example.org/onto/prop/google_looker_instance_additional_standard_user_count">
    <rdfs:label>additional_standard_user_count</rdfs:label>
    <rdfs:comment>Number of additional Standard Users to allocate to the Looker Instance.</rdfs:comment>
    <rdfs:domain rdf:resource="http://example.org/onto/class/google_looker_instance"/>
    <rdfs:range rdf:resource="http://www.w3.org/2001/XMLSchema#string"/>
  </owl:DatatypeProperty>
  <owl:DatatypeProperty rdf:about="http://example.org/onto/prop/google_looker_instance_additional_viewer_user_count">
    <rdfs:label>additional_viewer_user_count</rdfs:label>
    <rdfs:comment>Number of additional Viewer Users to allocate to the Looker Instance.</rdfs:comment>
    <rdfs:domain rdf:resource="http://example.org/onto/class/google_looker_instance"/>
    <rdfs:range rdf:resource="http://www.w3.org/2001/XMLSchema#string"/>
  </owl:DatatypeProperty>
</rdf:RDF>
