<?xml version="1.0" encoding="UTF-8"?>
<rdf:RDF
  xmlns:rdf="http://www.w3.org/1999/02/22-rdf-syntax-ns#"
  xmlns:rdfs="http://www.w3.org/2000/01/rdf-schema#"
  xmlns:owl="http://www.w3.org/2002/07/owl#"
  xmlns:xsd="http://www.w3.org/2001/XMLSchema#"
  xml:base="http://example.org/onto/">
  <owl:Class rdf:about="http://example.org/onto/class/google_scc_v2_project_mute_config">
    <rdfs:label>google_scc_v2_project_mute_config</rdfs:label>
    <rdfs:comment>#
#     ***     AUTO GENERATED CODE    ***    Type: MMv1     ***
#
# ----------------------------------------------------------------------------
#
#     This code is generated by Magic Modules using the following:
#
#     Configuration: https:#github.com/GoogleCloudPlatform/magic-modules/tree/main/mmv1/products/securitycenterv2/ProjectMuteConfig.yaml
#     Template:      https:#github.com/GoogleCloudPlatform/magic-modules/tree/main/mmv1/templates/terraform/resource.html.markdown.tmpl
#
#     DO NOT EDIT this file directly. Any changes made to this file will be
#     overwritten during the next generation cycle.
#
# ----------------------------------------------------------------------------
subcategory: "Security Command Center (SCC) v2 API"
description: |-
  Mute Findings is a volume management feature in Security Command Center
  that lets you manually or programmatically hide irrelevant findings,
  and create filters to automatically silence existing and future
  findings based on criteria you specify.
---</rdfs:comment>
  </owl:Class>
  <owl:DatatypeProperty rdf:about="http://example.org/onto/prop/google_scc_v2_project_mute_config_create_time">
    <rdfs:label>create_time</rdfs:label>
    <rdfs:comment>The time at which the mute config was created. This field is set by
the server and will be ignored if provided on config creation.</rdfs:comment>
    <rdfs:domain rdf:resource="http://example.org/onto/class/google_scc_v2_project_mute_config"/>
    <rdfs:range rdf:resource="http://www.w3.org/2001/XMLSchema#string"/>
  </owl:DatatypeProperty>
  <owl:DatatypeProperty rdf:about="http://example.org/onto/prop/google_scc_v2_project_mute_config_description">
    <rdfs:label>description</rdfs:label>
    <rdfs:comment>A description of the mute config.</rdfs:comment>
    <rdfs:domain rdf:resource="http://example.org/onto/class/google_scc_v2_project_mute_config"/>
    <rdfs:range rdf:resource="http://www.w3.org/2001/XMLSchema#string"/>
  </owl:DatatypeProperty>
  <owl:DatatypeProperty rdf:about="http://example.org/onto/prop/google_scc_v2_project_mute_config_filter">
    <rdfs:label>filter</rdfs:label>
    <rdfs:comment>An expression that defines the filter to apply across create/update
events of findings. While creating a filter string, be mindful of
the scope in which the mute configuration is being created. E.g.,
If a filter contains project = X but is created under the
project = Y scope, it might not match any findings.</rdfs:comment>
    <rdfs:domain rdf:resource="http://example.org/onto/class/google_scc_v2_project_mute_config"/>
    <rdfs:range rdf:resource="http://www.w3.org/2001/XMLSchema#string"/>
  </owl:DatatypeProperty>
  <owl:DatatypeProperty rdf:about="http://example.org/onto/prop/google_scc_v2_project_mute_config_id">
    <rdfs:label>id</rdfs:label>
    <rdfs:domain rdf:resource="http://example.org/onto/class/google_scc_v2_project_mute_config"/>
    <rdfs:range rdf:resource="http://www.w3.org/2001/XMLSchema#string"/>
  </owl:DatatypeProperty>
  <owl:DatatypeProperty rdf:about="http://example.org/onto/prop/google_scc_v2_project_mute_config_location">
    <rdfs:label>location</rdfs:label>
    <rdfs:comment>location Id is provided by project. If not provided, Use global as default.</rdfs:comment>
    <rdfs:domain rdf:resource="http://example.org/onto/class/google_scc_v2_project_mute_config"/>
    <rdfs:range rdf:resource="http://www.w3.org/2001/XMLSchema#string"/>
  </owl:DatatypeProperty>
  <owl:DatatypeProperty rdf:about="http://example.org/onto/prop/google_scc_v2_project_mute_config_most_recent_editor">
    <rdfs:label>most_recent_editor</rdfs:label>
    <rdfs:comment>Email address of the user who last edited the mute config. This
field is set by the server and will be ignored if provided on
config creation or update.</rdfs:comment>
    <rdfs:domain rdf:resource="http://example.org/onto/class/google_scc_v2_project_mute_config"/>
    <rdfs:range rdf:resource="http://www.w3.org/2001/XMLSchema#string"/>
  </owl:DatatypeProperty>
  <owl:DatatypeProperty rdf:about="http://example.org/onto/prop/google_scc_v2_project_mute_config_mute_config_id">
    <rdfs:label>mute_config_id</rdfs:label>
    <rdfs:comment>Unique identifier provided by the client within the parent scope.</rdfs:comment>
    <rdfs:domain rdf:resource="http://example.org/onto/class/google_scc_v2_project_mute_config"/>
    <rdfs:range rdf:resource="http://www.w3.org/2001/XMLSchema#string"/>
  </owl:DatatypeProperty>
  <owl:DatatypeProperty rdf:about="http://example.org/onto/prop/google_scc_v2_project_mute_config_name">
    <rdfs:label>name</rdfs:label>
    <rdfs:comment>Name of the mute config. Its format is
projects/{project}/locations/global/muteConfigs/{configId},
folders/{folder}/locations/global/muteConfigs/{configId},
or organizations/{organization}/locations/global/muteConfigs/{configId}</rdfs:comment>
    <rdfs:domain rdf:resource="http://example.org/onto/class/google_scc_v2_project_mute_config"/>
    <rdfs:range rdf:resource="http://www.w3.org/2001/XMLSchema#string"/>
  </owl:DatatypeProperty>
  <owl:DatatypeProperty rdf:about="http://example.org/onto/prop/google_scc_v2_project_mute_config_project">
    <rdfs:label>project</rdfs:label>
    <rdfs:domain rdf:resource="http://example.org/onto/class/google_scc_v2_project_mute_config"/>
    <rdfs:range rdf:resource="http://www.w3.org/2001/XMLSchema#string"/>
  </owl:DatatypeProperty>
  <owl:DatatypeProperty rdf:about="http://example.org/onto/prop/google_scc_v2_project_mute_config_type">
    <rdfs:label>type</rdfs:label>
    <rdfs:comment>The type of the mute config.</rdfs:comment>
    <rdfs:domain rdf:resource="http://example.org/onto/class/google_scc_v2_project_mute_config"/>
    <rdfs:range rdf:resource="http://www.w3.org/2001/XMLSchema#string"/>
  </owl:DatatypeProperty>
  <owl:DatatypeProperty rdf:about="http://example.org/onto/prop/google_scc_v2_project_mute_config_update_time">
    <rdfs:label>update_time</rdfs:label>
    <rdfs:comment>Output only. The most recent time at which the mute config was
updated. This field is set by the server and will be ignored if
provided on config creation or update.</rdfs:comment>
    <rdfs:domain rdf:resource="http://example.org/onto/class/google_scc_v2_project_mute_config"/>
    <rdfs:range rdf:resource="http://www.w3.org/2001/XMLSchema#string"/>
  </owl:DatatypeProperty>
  <owl:DatatypeProperty rdf:about="http://example.org/onto/prop/google_scc_v2_project_mute_config_create">
    <rdfs:label>create</rdfs:label>
    <rdfs:domain rdf:resource="http://example.org/onto/class/google_scc_v2_project_mute_config"/>
    <rdfs:range rdf:resource="http://www.w3.org/2001/XMLSchema#string"/>
  </owl:DatatypeProperty>
  <owl:DatatypeProperty rdf:about="http://example.org/onto/prop/google_scc_v2_project_mute_config_delete">
    <rdfs:label>delete</rdfs:label>
    <rdfs:domain rdf:resource="http://example.org/onto/class/google_scc_v2_project_mute_config"/>
    <rdfs:range rdf:resource="http://www.w3.org/2001/XMLSchema#string"/>
  </owl:DatatypeProperty>
  <owl:DatatypeProperty rdf:about="http://example.org/onto/prop/google_scc_v2_project_mute_config_update">
    <rdfs:label>update</rdfs:label>
    <rdfs:domain rdf:resource="http://example.org/onto/class/google_scc_v2_project_mute_config"/>
    <rdfs:range rdf:resource="http://www.w3.org/2001/XMLSchema#string"/>
  </owl:DatatypeProperty>
</rdf:RDF>
