<?xml version="1.0" encoding="UTF-8"?>
<rdf:RDF
  xmlns:rdf="http://www.w3.org/1999/02/22-rdf-syntax-ns#"
  xmlns:rdfs="http://www.w3.org/2000/01/rdf-schema#"
  xmlns:owl="http://www.w3.org/2002/07/owl#"
  xmlns:xsd="http://www.w3.org/2001/XMLSchema#"
  xml:base="http://example.org/onto/">
  <owl:Class rdf:about="http://example.org/onto/class/google_compute_security_policy">
    <rdfs:label>google_compute_security_policy</rdfs:label>
    <rdfs:comment>#
#     ***     AUTO GENERATED CODE    ***    Type: Handwritten     ***
#
# ----------------------------------------------------------------------------
#
#     This code is generated by Magic Modules using the following:
#
#     Source file: https://github.com/GoogleCloudPlatform/magic-modules/tree/main/mmv1/third_party/terraform/website/docs/r/compute_security_policy.html.markdown
#
#     DO NOT EDIT this file directly. Any changes made to this file will be
#     overwritten during the next generation cycle.
#
# ----------------------------------------------------------------------------
subcategory: "Compute Engine"
description: |-
  Creates a Security Policy resource for Google Compute Engine.
---</rdfs:comment>
  </owl:Class>
  <owl:DatatypeProperty rdf:about="http://example.org/onto/prop/google_compute_security_policy_description">
    <rdfs:label>description</rdfs:label>
    <rdfs:comment>An optional description of this security policy. Max size is 2048.</rdfs:comment>
    <rdfs:domain rdf:resource="http://example.org/onto/class/google_compute_security_policy"/>
    <rdfs:range rdf:resource="http://www.w3.org/2001/XMLSchema#string"/>
  </owl:DatatypeProperty>
  <owl:DatatypeProperty rdf:about="http://example.org/onto/prop/google_compute_security_policy_effective_labels">
    <rdfs:label>effective_labels</rdfs:label>
    <rdfs:comment>All of labels (key/value pairs) present on the resource in GCP, including the labels configured through Terraform, other clients and services.</rdfs:comment>
    <rdfs:domain rdf:resource="http://example.org/onto/class/google_compute_security_policy"/>
    <rdfs:range rdf:resource="http://www.w3.org/2001/XMLSchema#string"/>
  </owl:DatatypeProperty>
  <owl:DatatypeProperty rdf:about="http://example.org/onto/prop/google_compute_security_policy_fingerprint">
    <rdfs:label>fingerprint</rdfs:label>
    <rdfs:comment>Fingerprint of this resource.</rdfs:comment>
    <rdfs:domain rdf:resource="http://example.org/onto/class/google_compute_security_policy"/>
    <rdfs:range rdf:resource="http://www.w3.org/2001/XMLSchema#string"/>
  </owl:DatatypeProperty>
  <owl:DatatypeProperty rdf:about="http://example.org/onto/prop/google_compute_security_policy_id">
    <rdfs:label>id</rdfs:label>
    <rdfs:domain rdf:resource="http://example.org/onto/class/google_compute_security_policy"/>
    <rdfs:range rdf:resource="http://www.w3.org/2001/XMLSchema#string"/>
  </owl:DatatypeProperty>
  <owl:DatatypeProperty rdf:about="http://example.org/onto/prop/google_compute_security_policy_label_fingerprint">
    <rdfs:label>label_fingerprint</rdfs:label>
    <rdfs:comment>The unique fingerprint of the labels.</rdfs:comment>
    <rdfs:domain rdf:resource="http://example.org/onto/class/google_compute_security_policy"/>
    <rdfs:range rdf:resource="http://www.w3.org/2001/XMLSchema#string"/>
  </owl:DatatypeProperty>
  <owl:DatatypeProperty rdf:about="http://example.org/onto/prop/google_compute_security_policy_labels">
    <rdfs:label>labels</rdfs:label>
    <rdfs:comment>Labels to apply to this address.  A list of key->value pairs.


**Note**: This field is non-authoritative, and will only manage the labels present in your configuration.
Please refer to the field 'effective_labels' for all of the labels present on the resource.</rdfs:comment>
    <rdfs:domain rdf:resource="http://example.org/onto/class/google_compute_security_policy"/>
    <rdfs:range rdf:resource="http://www.w3.org/2001/XMLSchema#string"/>
  </owl:DatatypeProperty>
  <owl:DatatypeProperty rdf:about="http://example.org/onto/prop/google_compute_security_policy_name">
    <rdfs:label>name</rdfs:label>
    <rdfs:comment>The name of the security policy.</rdfs:comment>
    <rdfs:domain rdf:resource="http://example.org/onto/class/google_compute_security_policy"/>
    <rdfs:range rdf:resource="http://www.w3.org/2001/XMLSchema#string"/>
  </owl:DatatypeProperty>
  <owl:DatatypeProperty rdf:about="http://example.org/onto/prop/google_compute_security_policy_project">
    <rdfs:label>project</rdfs:label>
    <rdfs:comment>The project in which the resource belongs. If it is not provided, the provider project is used.</rdfs:comment>
    <rdfs:domain rdf:resource="http://example.org/onto/class/google_compute_security_policy"/>
    <rdfs:range rdf:resource="http://www.w3.org/2001/XMLSchema#string"/>
  </owl:DatatypeProperty>
  <owl:DatatypeProperty rdf:about="http://example.org/onto/prop/google_compute_security_policy_self_link">
    <rdfs:label>self_link</rdfs:label>
    <rdfs:comment>The URI of the created resource.</rdfs:comment>
    <rdfs:domain rdf:resource="http://example.org/onto/class/google_compute_security_policy"/>
    <rdfs:range rdf:resource="http://www.w3.org/2001/XMLSchema#string"/>
  </owl:DatatypeProperty>
  <owl:DatatypeProperty rdf:about="http://example.org/onto/prop/google_compute_security_policy_terraform_labels">
    <rdfs:label>terraform_labels</rdfs:label>
    <rdfs:comment>The combination of labels configured directly on the resource and default labels configured on the provider.</rdfs:comment>
    <rdfs:domain rdf:resource="http://example.org/onto/class/google_compute_security_policy"/>
    <rdfs:range rdf:resource="http://www.w3.org/2001/XMLSchema#string"/>
  </owl:DatatypeProperty>
  <owl:DatatypeProperty rdf:about="http://example.org/onto/prop/google_compute_security_policy_type">
    <rdfs:label>type</rdfs:label>
    <rdfs:comment>The type indicates the intended use of the security policy. CLOUD_ARMOR - Cloud Armor backend security policies can be configured to filter incoming HTTP requests targeting backend services. They filter requests before they hit the origin servers. CLOUD_ARMOR_EDGE - Cloud Armor edge security policies can be configured to filter incoming HTTP requests targeting backend services (including Cloud CDN-enabled) as well as backend buckets (Cloud Storage). They filter requests before the request is served from Google's cache.</rdfs:comment>
    <rdfs:domain rdf:resource="http://example.org/onto/class/google_compute_security_policy"/>
    <rdfs:range rdf:resource="http://www.w3.org/2001/XMLSchema#string"/>
  </owl:DatatypeProperty>
  <owl:DatatypeProperty rdf:about="http://example.org/onto/prop/google_compute_security_policy_enable">
    <rdfs:label>enable</rdfs:label>
    <rdfs:comment>If set to true, enables CAAP for L7 DDoS detection.</rdfs:comment>
    <rdfs:domain rdf:resource="http://example.org/onto/class/google_compute_security_policy"/>
    <rdfs:range rdf:resource="http://www.w3.org/2001/XMLSchema#string"/>
  </owl:DatatypeProperty>
  <owl:DatatypeProperty rdf:about="http://example.org/onto/prop/google_compute_security_policy_rule_visibility">
    <rdfs:label>rule_visibility</rdfs:label>
    <rdfs:comment>Rule visibility. Supported values include: "STANDARD", "PREMIUM".</rdfs:comment>
    <rdfs:domain rdf:resource="http://example.org/onto/class/google_compute_security_policy"/>
    <rdfs:range rdf:resource="http://www.w3.org/2001/XMLSchema#string"/>
  </owl:DatatypeProperty>
  <owl:DatatypeProperty rdf:about="http://example.org/onto/prop/google_compute_security_policy_auto_deploy_confidence_threshold">
    <rdfs:label>auto_deploy_confidence_threshold</rdfs:label>
    <rdfs:domain rdf:resource="http://example.org/onto/class/google_compute_security_policy"/>
    <rdfs:range rdf:resource="http://www.w3.org/2001/XMLSchema#string"/>
  </owl:DatatypeProperty>
  <owl:DatatypeProperty rdf:about="http://example.org/onto/prop/google_compute_security_policy_auto_deploy_expiration_sec">
    <rdfs:label>auto_deploy_expiration_sec</rdfs:label>
    <rdfs:domain rdf:resource="http://example.org/onto/class/google_compute_security_policy"/>
    <rdfs:range rdf:resource="http://www.w3.org/2001/XMLSchema#string"/>
  </owl:DatatypeProperty>
  <owl:DatatypeProperty rdf:about="http://example.org/onto/prop/google_compute_security_policy_auto_deploy_impacted_baseline_threshold">
    <rdfs:label>auto_deploy_impacted_baseline_threshold</rdfs:label>
    <rdfs:domain rdf:resource="http://example.org/onto/class/google_compute_security_policy"/>
    <rdfs:range rdf:resource="http://www.w3.org/2001/XMLSchema#string"/>
  </owl:DatatypeProperty>
  <owl:DatatypeProperty rdf:about="http://example.org/onto/prop/google_compute_security_policy_auto_deploy_load_threshold">
    <rdfs:label>auto_deploy_load_threshold</rdfs:label>
    <rdfs:domain rdf:resource="http://example.org/onto/class/google_compute_security_policy"/>
    <rdfs:range rdf:resource="http://www.w3.org/2001/XMLSchema#string"/>
  </owl:DatatypeProperty>
  <owl:DatatypeProperty rdf:about="http://example.org/onto/prop/google_compute_security_policy_detection_absolute_qps">
    <rdfs:label>detection_absolute_qps</rdfs:label>
    <rdfs:domain rdf:resource="http://example.org/onto/class/google_compute_security_policy"/>
    <rdfs:range rdf:resource="http://www.w3.org/2001/XMLSchema#string"/>
  </owl:DatatypeProperty>
  <owl:DatatypeProperty rdf:about="http://example.org/onto/prop/google_compute_security_policy_detection_load_threshold">
    <rdfs:label>detection_load_threshold</rdfs:label>
    <rdfs:domain rdf:resource="http://example.org/onto/class/google_compute_security_policy"/>
    <rdfs:range rdf:resource="http://www.w3.org/2001/XMLSchema#string"/>
  </owl:DatatypeProperty>
  <owl:DatatypeProperty rdf:about="http://example.org/onto/prop/google_compute_security_policy_detection_relative_to_baseline_qps">
    <rdfs:label>detection_relative_to_baseline_qps</rdfs:label>
    <rdfs:domain rdf:resource="http://example.org/onto/class/google_compute_security_policy"/>
    <rdfs:range rdf:resource="http://www.w3.org/2001/XMLSchema#string"/>
  </owl:DatatypeProperty>
  <owl:DatatypeProperty rdf:about="http://example.org/onto/prop/google_compute_security_policy_name">
    <rdfs:label>name</rdfs:label>
    <rdfs:comment>The name must be 1-63 characters long, and comply with RFC1035. The name must be unique within the security policy.</rdfs:comment>
    <rdfs:domain rdf:resource="http://example.org/onto/class/google_compute_security_policy"/>
    <rdfs:range rdf:resource="http://www.w3.org/2001/XMLSchema#string"/>
  </owl:DatatypeProperty>
  <owl:DatatypeProperty rdf:about="http://example.org/onto/prop/google_compute_security_policy_enable_each_unique_value">
    <rdfs:label>enable_each_unique_value</rdfs:label>
    <rdfs:comment>If enabled, traffic matching each unique value for the specified type constitutes a separate traffic unit. It can only be set to true if value is empty.</rdfs:comment>
    <rdfs:domain rdf:resource="http://example.org/onto/class/google_compute_security_policy"/>
    <rdfs:range rdf:resource="http://www.w3.org/2001/XMLSchema#string"/>
  </owl:DatatypeProperty>
  <owl:DatatypeProperty rdf:about="http://example.org/onto/prop/google_compute_security_policy_type">
    <rdfs:label>type</rdfs:label>
    <rdfs:comment>Type of this configuration.</rdfs:comment>
    <rdfs:domain rdf:resource="http://example.org/onto/class/google_compute_security_policy"/>
    <rdfs:range rdf:resource="http://www.w3.org/2001/XMLSchema#string"/>
  </owl:DatatypeProperty>
  <owl:DatatypeProperty rdf:about="http://example.org/onto/prop/google_compute_security_policy_value">
    <rdfs:label>value</rdfs:label>
    <rdfs:comment>Requests that match this value constitute a granular traffic unit.</rdfs:comment>
    <rdfs:domain rdf:resource="http://example.org/onto/class/google_compute_security_policy"/>
    <rdfs:range rdf:resource="http://www.w3.org/2001/XMLSchema#string"/>
  </owl:DatatypeProperty>
  <owl:DatatypeProperty rdf:about="http://example.org/onto/prop/google_compute_security_policy_json_parsing">
    <rdfs:label>json_parsing</rdfs:label>
    <rdfs:comment>JSON body parsing. Supported values include: "DISABLED", "STANDARD".</rdfs:comment>
    <rdfs:domain rdf:resource="http://example.org/onto/class/google_compute_security_policy"/>
    <rdfs:range rdf:resource="http://www.w3.org/2001/XMLSchema#string"/>
  </owl:DatatypeProperty>
  <owl:DatatypeProperty rdf:about="http://example.org/onto/prop/google_compute_security_policy_log_level">
    <rdfs:label>log_level</rdfs:label>
    <rdfs:comment>Logging level. Supported values include: "NORMAL", "VERBOSE".</rdfs:comment>
    <rdfs:domain rdf:resource="http://example.org/onto/class/google_compute_security_policy"/>
    <rdfs:range rdf:resource="http://www.w3.org/2001/XMLSchema#string"/>
  </owl:DatatypeProperty>
  <owl:DatatypeProperty rdf:about="http://example.org/onto/prop/google_compute_security_policy_user_ip_request_headers">
    <rdfs:label>user_ip_request_headers</rdfs:label>
    <rdfs:comment>An optional list of case-insensitive request header names to use for resolving the callers client IP address.</rdfs:comment>
    <rdfs:domain rdf:resource="http://example.org/onto/class/google_compute_security_policy"/>
    <rdfs:range rdf:resource="http://www.w3.org/2001/XMLSchema#string"/>
  </owl:DatatypeProperty>
  <owl:DatatypeProperty rdf:about="http://example.org/onto/prop/google_compute_security_policy_content_types">
    <rdfs:label>content_types</rdfs:label>
    <rdfs:comment>A list of custom Content-Type header values to apply the JSON parsing.</rdfs:comment>
    <rdfs:domain rdf:resource="http://example.org/onto/class/google_compute_security_policy"/>
    <rdfs:range rdf:resource="http://www.w3.org/2001/XMLSchema#string"/>
  </owl:DatatypeProperty>
  <owl:DatatypeProperty rdf:about="http://example.org/onto/prop/google_compute_security_policy_redirect_site_key">
    <rdfs:label>redirect_site_key</rdfs:label>
    <rdfs:comment>A field to supply a reCAPTCHA site key to be used for all the rules using the redirect action with the type of GOOGLE_RECAPTCHA under the security policy. The specified site key needs to be created from the reCAPTCHA API. The user is responsible for the validity of the specified site key. If not specified, a Google-managed site key is used.</rdfs:comment>
    <rdfs:domain rdf:resource="http://example.org/onto/class/google_compute_security_policy"/>
    <rdfs:range rdf:resource="http://www.w3.org/2001/XMLSchema#string"/>
  </owl:DatatypeProperty>
  <owl:DatatypeProperty rdf:about="http://example.org/onto/prop/google_compute_security_policy_action">
    <rdfs:label>action</rdfs:label>
    <rdfs:comment>Action to take when match matches the request.</rdfs:comment>
    <rdfs:domain rdf:resource="http://example.org/onto/class/google_compute_security_policy"/>
    <rdfs:range rdf:resource="http://www.w3.org/2001/XMLSchema#string"/>
  </owl:DatatypeProperty>
  <owl:DatatypeProperty rdf:about="http://example.org/onto/prop/google_compute_security_policy_description">
    <rdfs:label>description</rdfs:label>
    <rdfs:comment>An optional description of this rule. Max size is 64.</rdfs:comment>
    <rdfs:domain rdf:resource="http://example.org/onto/class/google_compute_security_policy"/>
    <rdfs:range rdf:resource="http://www.w3.org/2001/XMLSchema#string"/>
  </owl:DatatypeProperty>
  <owl:DatatypeProperty rdf:about="http://example.org/onto/prop/google_compute_security_policy_preview">
    <rdfs:label>preview</rdfs:label>
    <rdfs:comment>When set to true, the action specified above is not enforced. Stackdriver logs for requests that trigger a preview action are annotated as such.</rdfs:comment>
    <rdfs:domain rdf:resource="http://example.org/onto/class/google_compute_security_policy"/>
    <rdfs:range rdf:resource="http://www.w3.org/2001/XMLSchema#string"/>
  </owl:DatatypeProperty>
  <owl:DatatypeProperty rdf:about="http://example.org/onto/prop/google_compute_security_policy_priority">
    <rdfs:label>priority</rdfs:label>
    <rdfs:comment>An unique positive integer indicating the priority of evaluation for a rule. Rules are evaluated from highest priority (lowest numerically) to lowest priority (highest numerically) in order.</rdfs:comment>
    <rdfs:domain rdf:resource="http://example.org/onto/class/google_compute_security_policy"/>
    <rdfs:range rdf:resource="http://www.w3.org/2001/XMLSchema#string"/>
  </owl:DatatypeProperty>
  <owl:DatatypeProperty rdf:about="http://example.org/onto/prop/google_compute_security_policy_header_name">
    <rdfs:label>header_name</rdfs:label>
    <rdfs:comment>The name of the header to set.</rdfs:comment>
    <rdfs:domain rdf:resource="http://example.org/onto/class/google_compute_security_policy"/>
    <rdfs:range rdf:resource="http://www.w3.org/2001/XMLSchema#string"/>
  </owl:DatatypeProperty>
  <owl:DatatypeProperty rdf:about="http://example.org/onto/prop/google_compute_security_policy_header_value">
    <rdfs:label>header_value</rdfs:label>
    <rdfs:comment>The value to set the named header to.</rdfs:comment>
    <rdfs:domain rdf:resource="http://example.org/onto/class/google_compute_security_policy"/>
    <rdfs:range rdf:resource="http://www.w3.org/2001/XMLSchema#string"/>
  </owl:DatatypeProperty>
  <owl:DatatypeProperty rdf:about="http://example.org/onto/prop/google_compute_security_policy_versioned_expr">
    <rdfs:label>versioned_expr</rdfs:label>
    <rdfs:comment>Predefined rule expression. If this field is specified, config must also be specified. Available options:   SRC_IPS_V1: Must specify the corresponding src_ip_ranges field in config.</rdfs:comment>
    <rdfs:domain rdf:resource="http://example.org/onto/class/google_compute_security_policy"/>
    <rdfs:range rdf:resource="http://www.w3.org/2001/XMLSchema#string"/>
  </owl:DatatypeProperty>
  <owl:DatatypeProperty rdf:about="http://example.org/onto/prop/google_compute_security_policy_src_ip_ranges">
    <rdfs:label>src_ip_ranges</rdfs:label>
    <rdfs:comment>Set of IP addresses or ranges (IPV4 or IPV6) in CIDR notation to match against inbound traffic. There is a limit of 10 IP ranges per rule. A value of '*' matches all IPs (can be used to override the default behavior).</rdfs:comment>
    <rdfs:domain rdf:resource="http://example.org/onto/class/google_compute_security_policy"/>
    <rdfs:range rdf:resource="http://www.w3.org/2001/XMLSchema#string"/>
  </owl:DatatypeProperty>
  <owl:DatatypeProperty rdf:about="http://example.org/onto/prop/google_compute_security_policy_expression">
    <rdfs:label>expression</rdfs:label>
    <rdfs:comment>Textual representation of an expression in Common Expression Language syntax. The application context of the containing message determines which well-known feature set of CEL is supported.</rdfs:comment>
    <rdfs:domain rdf:resource="http://example.org/onto/class/google_compute_security_policy"/>
    <rdfs:range rdf:resource="http://www.w3.org/2001/XMLSchema#string"/>
  </owl:DatatypeProperty>
  <owl:DatatypeProperty rdf:about="http://example.org/onto/prop/google_compute_security_policy_action_token_site_keys">
    <rdfs:label>action_token_site_keys</rdfs:label>
    <rdfs:comment>A list of site keys to be used during the validation of reCAPTCHA action-tokens. The provided site keys need to be created from reCAPTCHA API under the same project where the security policy is created</rdfs:comment>
    <rdfs:domain rdf:resource="http://example.org/onto/class/google_compute_security_policy"/>
    <rdfs:range rdf:resource="http://www.w3.org/2001/XMLSchema#string"/>
  </owl:DatatypeProperty>
  <owl:DatatypeProperty rdf:about="http://example.org/onto/prop/google_compute_security_policy_session_token_site_keys">
    <rdfs:label>session_token_site_keys</rdfs:label>
    <rdfs:comment>A list of site keys to be used during the validation of reCAPTCHA session-tokens. The provided site keys need to be created from reCAPTCHA API under the same project where the security policy is created.</rdfs:comment>
    <rdfs:domain rdf:resource="http://example.org/onto/class/google_compute_security_policy"/>
    <rdfs:range rdf:resource="http://www.w3.org/2001/XMLSchema#string"/>
  </owl:DatatypeProperty>
  <owl:DatatypeProperty rdf:about="http://example.org/onto/prop/google_compute_security_policy_target_rule_ids">
    <rdfs:label>target_rule_ids</rdfs:label>
    <rdfs:comment>A list of target rule IDs under the WAF rule set to apply the preconfigured WAF exclusion. If omitted, it refers to all the rule IDs under the WAF rule set.</rdfs:comment>
    <rdfs:domain rdf:resource="http://example.org/onto/class/google_compute_security_policy"/>
    <rdfs:range rdf:resource="http://www.w3.org/2001/XMLSchema#string"/>
  </owl:DatatypeProperty>
  <owl:DatatypeProperty rdf:about="http://example.org/onto/prop/google_compute_security_policy_target_rule_set">
    <rdfs:label>target_rule_set</rdfs:label>
    <rdfs:comment>Target WAF rule set to apply the preconfigured WAF exclusion.</rdfs:comment>
    <rdfs:domain rdf:resource="http://example.org/onto/class/google_compute_security_policy"/>
    <rdfs:range rdf:resource="http://www.w3.org/2001/XMLSchema#string"/>
  </owl:DatatypeProperty>
  <owl:DatatypeProperty rdf:about="http://example.org/onto/prop/google_compute_security_policy_operator">
    <rdfs:label>operator</rdfs:label>
    <rdfs:comment>You can specify an exact match or a partial match by using a field operator and a field value. Available options: EQUALS: The operator matches if the field value equals the specified value. STARTS_WITH: The operator matches if the field value starts with the specified value. ENDS_WITH: The operator matches if the field value ends with the specified value. CONTAINS: The operator matches if the field value contains the specified value. EQUALS_ANY: The operator matches if the field value is any value.</rdfs:comment>
    <rdfs:domain rdf:resource="http://example.org/onto/class/google_compute_security_policy"/>
    <rdfs:range rdf:resource="http://www.w3.org/2001/XMLSchema#string"/>
  </owl:DatatypeProperty>
  <owl:DatatypeProperty rdf:about="http://example.org/onto/prop/google_compute_security_policy_value">
    <rdfs:label>value</rdfs:label>
    <rdfs:comment>A request field matching the specified value will be excluded from inspection during preconfigured WAF evaluation. The field value must be given if the field operator is not EQUALS_ANY, and cannot be given if the field operator is EQUALS_ANY.</rdfs:comment>
    <rdfs:domain rdf:resource="http://example.org/onto/class/google_compute_security_policy"/>
    <rdfs:range rdf:resource="http://www.w3.org/2001/XMLSchema#string"/>
  </owl:DatatypeProperty>
  <owl:DatatypeProperty rdf:about="http://example.org/onto/prop/google_compute_security_policy_operator">
    <rdfs:label>operator</rdfs:label>
    <rdfs:comment>You can specify an exact match or a partial match by using a field operator and a field value. Available options: EQUALS: The operator matches if the field value equals the specified value. STARTS_WITH: The operator matches if the field value starts with the specified value. ENDS_WITH: The operator matches if the field value ends with the specified value. CONTAINS: The operator matches if the field value contains the specified value. EQUALS_ANY: The operator matches if the field value is any value.</rdfs:comment>
    <rdfs:domain rdf:resource="http://example.org/onto/class/google_compute_security_policy"/>
    <rdfs:range rdf:resource="http://www.w3.org/2001/XMLSchema#string"/>
  </owl:DatatypeProperty>
  <owl:DatatypeProperty rdf:about="http://example.org/onto/prop/google_compute_security_policy_value">
    <rdfs:label>value</rdfs:label>
    <rdfs:comment>A request field matching the specified value will be excluded from inspection during preconfigured WAF evaluation. The field value must be given if the field operator is not EQUALS_ANY, and cannot be given if the field operator is EQUALS_ANY.</rdfs:comment>
    <rdfs:domain rdf:resource="http://example.org/onto/class/google_compute_security_policy"/>
    <rdfs:range rdf:resource="http://www.w3.org/2001/XMLSchema#string"/>
  </owl:DatatypeProperty>
  <owl:DatatypeProperty rdf:about="http://example.org/onto/prop/google_compute_security_policy_operator">
    <rdfs:label>operator</rdfs:label>
    <rdfs:comment>You can specify an exact match or a partial match by using a field operator and a field value. Available options: EQUALS: The operator matches if the field value equals the specified value. STARTS_WITH: The operator matches if the field value starts with the specified value. ENDS_WITH: The operator matches if the field value ends with the specified value. CONTAINS: The operator matches if the field value contains the specified value. EQUALS_ANY: The operator matches if the field value is any value.</rdfs:comment>
    <rdfs:domain rdf:resource="http://example.org/onto/class/google_compute_security_policy"/>
    <rdfs:range rdf:resource="http://www.w3.org/2001/XMLSchema#string"/>
  </owl:DatatypeProperty>
  <owl:DatatypeProperty rdf:about="http://example.org/onto/prop/google_compute_security_policy_value">
    <rdfs:label>value</rdfs:label>
    <rdfs:comment>A request field matching the specified value will be excluded from inspection during preconfigured WAF evaluation. The field value must be given if the field operator is not EQUALS_ANY, and cannot be given if the field operator is EQUALS_ANY.</rdfs:comment>
    <rdfs:domain rdf:resource="http://example.org/onto/class/google_compute_security_policy"/>
    <rdfs:range rdf:resource="http://www.w3.org/2001/XMLSchema#string"/>
  </owl:DatatypeProperty>
  <owl:DatatypeProperty rdf:about="http://example.org/onto/prop/google_compute_security_policy_operator">
    <rdfs:label>operator</rdfs:label>
    <rdfs:comment>You can specify an exact match or a partial match by using a field operator and a field value. Available options: EQUALS: The operator matches if the field value equals the specified value. STARTS_WITH: The operator matches if the field value starts with the specified value. ENDS_WITH: The operator matches if the field value ends with the specified value. CONTAINS: The operator matches if the field value contains the specified value. EQUALS_ANY: The operator matches if the field value is any value.</rdfs:comment>
    <rdfs:domain rdf:resource="http://example.org/onto/class/google_compute_security_policy"/>
    <rdfs:range rdf:resource="http://www.w3.org/2001/XMLSchema#string"/>
  </owl:DatatypeProperty>
  <owl:DatatypeProperty rdf:about="http://example.org/onto/prop/google_compute_security_policy_value">
    <rdfs:label>value</rdfs:label>
    <rdfs:comment>A request field matching the specified value will be excluded from inspection during preconfigured WAF evaluation. The field value must be given if the field operator is not EQUALS_ANY, and cannot be given if the field operator is EQUALS_ANY.</rdfs:comment>
    <rdfs:domain rdf:resource="http://example.org/onto/class/google_compute_security_policy"/>
    <rdfs:range rdf:resource="http://www.w3.org/2001/XMLSchema#string"/>
  </owl:DatatypeProperty>
  <owl:DatatypeProperty rdf:about="http://example.org/onto/prop/google_compute_security_policy_ban_duration_sec">
    <rdfs:label>ban_duration_sec</rdfs:label>
    <rdfs:comment>Can only be specified if the action for the rule is "rate_based_ban". If specified, determines the time (in seconds) the traffic will continue to be banned by the rate limit after the rate falls below the threshold.</rdfs:comment>
    <rdfs:domain rdf:resource="http://example.org/onto/class/google_compute_security_policy"/>
    <rdfs:range rdf:resource="http://www.w3.org/2001/XMLSchema#string"/>
  </owl:DatatypeProperty>
  <owl:DatatypeProperty rdf:about="http://example.org/onto/prop/google_compute_security_policy_conform_action">
    <rdfs:label>conform_action</rdfs:label>
    <rdfs:comment>Action to take for requests that are under the configured rate limit threshold. Valid option is "allow" only.</rdfs:comment>
    <rdfs:domain rdf:resource="http://example.org/onto/class/google_compute_security_policy"/>
    <rdfs:range rdf:resource="http://www.w3.org/2001/XMLSchema#string"/>
  </owl:DatatypeProperty>
  <owl:DatatypeProperty rdf:about="http://example.org/onto/prop/google_compute_security_policy_enforce_on_key">
    <rdfs:label>enforce_on_key</rdfs:label>
    <rdfs:comment>Determines the key to enforce the rateLimitThreshold on</rdfs:comment>
    <rdfs:domain rdf:resource="http://example.org/onto/class/google_compute_security_policy"/>
    <rdfs:range rdf:resource="http://www.w3.org/2001/XMLSchema#string"/>
  </owl:DatatypeProperty>
  <owl:DatatypeProperty rdf:about="http://example.org/onto/prop/google_compute_security_policy_enforce_on_key_name">
    <rdfs:label>enforce_on_key_name</rdfs:label>
    <rdfs:comment>Rate limit key name applicable only for the following key types: HTTP_HEADER -- Name of the HTTP header whose value is taken as the key value. HTTP_COOKIE -- Name of the HTTP cookie whose value is taken as the key value.</rdfs:comment>
    <rdfs:domain rdf:resource="http://example.org/onto/class/google_compute_security_policy"/>
    <rdfs:range rdf:resource="http://www.w3.org/2001/XMLSchema#string"/>
  </owl:DatatypeProperty>
  <owl:DatatypeProperty rdf:about="http://example.org/onto/prop/google_compute_security_policy_exceed_action">
    <rdfs:label>exceed_action</rdfs:label>
    <rdfs:comment>Action to take for requests that are above the configured rate limit threshold, to either deny with a specified HTTP response code, or redirect to a different endpoint. Valid options are "deny()" where valid values for status are 403, 404, 429, and 502, and "redirect" where the redirect parameters come from exceedRedirectOptions below.</rdfs:comment>
    <rdfs:domain rdf:resource="http://example.org/onto/class/google_compute_security_policy"/>
    <rdfs:range rdf:resource="http://www.w3.org/2001/XMLSchema#string"/>
  </owl:DatatypeProperty>
  <owl:DatatypeProperty rdf:about="http://example.org/onto/prop/google_compute_security_policy_count">
    <rdfs:label>count</rdfs:label>
    <rdfs:comment>Number of HTTP(S) requests for calculating the threshold.</rdfs:comment>
    <rdfs:domain rdf:resource="http://example.org/onto/class/google_compute_security_policy"/>
    <rdfs:range rdf:resource="http://www.w3.org/2001/XMLSchema#string"/>
  </owl:DatatypeProperty>
  <owl:DatatypeProperty rdf:about="http://example.org/onto/prop/google_compute_security_policy_interval_sec">
    <rdfs:label>interval_sec</rdfs:label>
    <rdfs:comment>Interval over which the threshold is computed.</rdfs:comment>
    <rdfs:domain rdf:resource="http://example.org/onto/class/google_compute_security_policy"/>
    <rdfs:range rdf:resource="http://www.w3.org/2001/XMLSchema#string"/>
  </owl:DatatypeProperty>
  <owl:DatatypeProperty rdf:about="http://example.org/onto/prop/google_compute_security_policy_enforce_on_key_name">
    <rdfs:label>enforce_on_key_name</rdfs:label>
    <rdfs:comment>Rate limit key name applicable only for the following key types: HTTP_HEADER -- Name of the HTTP header whose value is taken as the key value. HTTP_COOKIE -- Name of the HTTP cookie whose value is taken as the key value.</rdfs:comment>
    <rdfs:domain rdf:resource="http://example.org/onto/class/google_compute_security_policy"/>
    <rdfs:range rdf:resource="http://www.w3.org/2001/XMLSchema#string"/>
  </owl:DatatypeProperty>
  <owl:DatatypeProperty rdf:about="http://example.org/onto/prop/google_compute_security_policy_enforce_on_key_type">
    <rdfs:label>enforce_on_key_type</rdfs:label>
    <rdfs:comment>Determines the key to enforce the rate_limit_threshold on</rdfs:comment>
    <rdfs:domain rdf:resource="http://example.org/onto/class/google_compute_security_policy"/>
    <rdfs:range rdf:resource="http://www.w3.org/2001/XMLSchema#string"/>
  </owl:DatatypeProperty>
  <owl:DatatypeProperty rdf:about="http://example.org/onto/prop/google_compute_security_policy_target">
    <rdfs:label>target</rdfs:label>
    <rdfs:comment>Target for the redirect action. This is required if the type is EXTERNAL_302 and cannot be specified for GOOGLE_RECAPTCHA.</rdfs:comment>
    <rdfs:domain rdf:resource="http://example.org/onto/class/google_compute_security_policy"/>
    <rdfs:range rdf:resource="http://www.w3.org/2001/XMLSchema#string"/>
  </owl:DatatypeProperty>
  <owl:DatatypeProperty rdf:about="http://example.org/onto/prop/google_compute_security_policy_type">
    <rdfs:label>type</rdfs:label>
    <rdfs:comment>Type of the redirect action.</rdfs:comment>
    <rdfs:domain rdf:resource="http://example.org/onto/class/google_compute_security_policy"/>
    <rdfs:range rdf:resource="http://www.w3.org/2001/XMLSchema#string"/>
  </owl:DatatypeProperty>
  <owl:DatatypeProperty rdf:about="http://example.org/onto/prop/google_compute_security_policy_count">
    <rdfs:label>count</rdfs:label>
    <rdfs:comment>Number of HTTP(S) requests for calculating the threshold.</rdfs:comment>
    <rdfs:domain rdf:resource="http://example.org/onto/class/google_compute_security_policy"/>
    <rdfs:range rdf:resource="http://www.w3.org/2001/XMLSchema#string"/>
  </owl:DatatypeProperty>
  <owl:DatatypeProperty rdf:about="http://example.org/onto/prop/google_compute_security_policy_interval_sec">
    <rdfs:label>interval_sec</rdfs:label>
    <rdfs:comment>Interval over which the threshold is computed.</rdfs:comment>
    <rdfs:domain rdf:resource="http://example.org/onto/class/google_compute_security_policy"/>
    <rdfs:range rdf:resource="http://www.w3.org/2001/XMLSchema#string"/>
  </owl:DatatypeProperty>
  <owl:DatatypeProperty rdf:about="http://example.org/onto/prop/google_compute_security_policy_target">
    <rdfs:label>target</rdfs:label>
    <rdfs:comment>Target for the redirect action. This is required if the type is EXTERNAL_302 and cannot be specified for GOOGLE_RECAPTCHA.</rdfs:comment>
    <rdfs:domain rdf:resource="http://example.org/onto/class/google_compute_security_policy"/>
    <rdfs:range rdf:resource="http://www.w3.org/2001/XMLSchema#string"/>
  </owl:DatatypeProperty>
  <owl:DatatypeProperty rdf:about="http://example.org/onto/prop/google_compute_security_policy_type">
    <rdfs:label>type</rdfs:label>
    <rdfs:comment>Type of the redirect action. Available options: EXTERNAL_302: Must specify the corresponding target field in config. GOOGLE_RECAPTCHA: Cannot specify target field in config.</rdfs:comment>
    <rdfs:domain rdf:resource="http://example.org/onto/class/google_compute_security_policy"/>
    <rdfs:range rdf:resource="http://www.w3.org/2001/XMLSchema#string"/>
  </owl:DatatypeProperty>
  <owl:DatatypeProperty rdf:about="http://example.org/onto/prop/google_compute_security_policy_create">
    <rdfs:label>create</rdfs:label>
    <rdfs:domain rdf:resource="http://example.org/onto/class/google_compute_security_policy"/>
    <rdfs:range rdf:resource="http://www.w3.org/2001/XMLSchema#string"/>
  </owl:DatatypeProperty>
  <owl:DatatypeProperty rdf:about="http://example.org/onto/prop/google_compute_security_policy_delete">
    <rdfs:label>delete</rdfs:label>
    <rdfs:domain rdf:resource="http://example.org/onto/class/google_compute_security_policy"/>
    <rdfs:range rdf:resource="http://www.w3.org/2001/XMLSchema#string"/>
  </owl:DatatypeProperty>
  <owl:DatatypeProperty rdf:about="http://example.org/onto/prop/google_compute_security_policy_update">
    <rdfs:label>update</rdfs:label>
    <rdfs:domain rdf:resource="http://example.org/onto/class/google_compute_security_policy"/>
    <rdfs:range rdf:resource="http://www.w3.org/2001/XMLSchema#string"/>
  </owl:DatatypeProperty>
</rdf:RDF>
