<?xml version="1.0" encoding="UTF-8"?>
<rdf:RDF
  xmlns:rdf="http://www.w3.org/1999/02/22-rdf-syntax-ns#"
  xmlns:rdfs="http://www.w3.org/2000/01/rdf-schema#"
  xmlns:owl="http://www.w3.org/2002/07/owl#"
  xmlns:xsd="http://www.w3.org/2001/XMLSchema#"
  xml:base="http://example.org/onto/">
  <owl:Class rdf:about="http://example.org/onto/class/google_sql_database_instance">
    <rdfs:label>google_sql_database_instance</rdfs:label>
    <rdfs:comment>#
#     ***     AUTO GENERATED CODE    ***    Type: Handwritten     ***
#
# ----------------------------------------------------------------------------
#
#     This code is generated by Magic Modules using the following:
#
#     Source file: https://github.com/GoogleCloudPlatform/magic-modules/tree/main/mmv1/third_party/terraform/website/docs/r/sql_database_instance.html.markdown
#
#     DO NOT EDIT this file directly. Any changes made to this file will be
#     overwritten during the next generation cycle.
#
# ----------------------------------------------------------------------------
subcategory: "Cloud SQL"
description: |-
  Creates a new SQL database instance in Google Cloud SQL.
---</rdfs:comment>
  </owl:Class>
  <owl:DatatypeProperty rdf:about="http://example.org/onto/prop/google_sql_database_instance_available_maintenance_versions">
    <rdfs:label>available_maintenance_versions</rdfs:label>
    <rdfs:comment>Available Maintenance versions.</rdfs:comment>
    <rdfs:domain rdf:resource="http://example.org/onto/class/google_sql_database_instance"/>
    <rdfs:range rdf:resource="http://www.w3.org/2001/XMLSchema#string"/>
  </owl:DatatypeProperty>
  <owl:DatatypeProperty rdf:about="http://example.org/onto/prop/google_sql_database_instance_backupdr_backup">
    <rdfs:label>backupdr_backup</rdfs:label>
    <rdfs:comment>The name of the BackupDR backup to restore from.</rdfs:comment>
    <rdfs:domain rdf:resource="http://example.org/onto/class/google_sql_database_instance"/>
    <rdfs:range rdf:resource="http://www.w3.org/2001/XMLSchema#string"/>
  </owl:DatatypeProperty>
  <owl:DatatypeProperty rdf:about="http://example.org/onto/prop/google_sql_database_instance_connection_name">
    <rdfs:label>connection_name</rdfs:label>
    <rdfs:comment>The connection name of the instance to be used in connection strings. For example, when connecting with Cloud SQL Proxy.</rdfs:comment>
    <rdfs:domain rdf:resource="http://example.org/onto/class/google_sql_database_instance"/>
    <rdfs:range rdf:resource="http://www.w3.org/2001/XMLSchema#string"/>
  </owl:DatatypeProperty>
  <owl:DatatypeProperty rdf:about="http://example.org/onto/prop/google_sql_database_instance_database_version">
    <rdfs:label>database_version</rdfs:label>
    <rdfs:comment>The MySQL, PostgreSQL or SQL Server (beta) version to use. Supported values include MYSQL_5_6, MYSQL_5_7, MYSQL_8_0, MYSQL_8_4, POSTGRES_9_6, POSTGRES_10, POSTGRES_11, POSTGRES_12, POSTGRES_13, POSTGRES_14, POSTGRES_15, POSTGRES_16, POSTGRES_17, SQLSERVER_2017_STANDARD, SQLSERVER_2017_ENTERPRISE, SQLSERVER_2017_EXPRESS, SQLSERVER_2017_WEB. Database Version Policies includes an up-to-date reference of supported versions.</rdfs:comment>
    <rdfs:domain rdf:resource="http://example.org/onto/class/google_sql_database_instance"/>
    <rdfs:range rdf:resource="http://www.w3.org/2001/XMLSchema#string"/>
  </owl:DatatypeProperty>
  <owl:DatatypeProperty rdf:about="http://example.org/onto/prop/google_sql_database_instance_deletion_protection">
    <rdfs:label>deletion_protection</rdfs:label>
    <rdfs:comment>Used to block Terraform from deleting a SQL Instance. Defaults to true.</rdfs:comment>
    <rdfs:domain rdf:resource="http://example.org/onto/class/google_sql_database_instance"/>
    <rdfs:range rdf:resource="http://www.w3.org/2001/XMLSchema#string"/>
  </owl:DatatypeProperty>
  <owl:DatatypeProperty rdf:about="http://example.org/onto/prop/google_sql_database_instance_dns_name">
    <rdfs:label>dns_name</rdfs:label>
    <rdfs:comment>The instance-level dns name of the instance for PSC instances or public IP CAS instances.</rdfs:comment>
    <rdfs:domain rdf:resource="http://example.org/onto/class/google_sql_database_instance"/>
    <rdfs:range rdf:resource="http://www.w3.org/2001/XMLSchema#string"/>
  </owl:DatatypeProperty>
  <owl:DatatypeProperty rdf:about="http://example.org/onto/prop/google_sql_database_instance_dns_names">
    <rdfs:label>dns_names</rdfs:label>
    <rdfs:comment>The list of DNS names used by this instance. Different connection types for an instance may have different DNS names. DNS names can apply to an individual instance or a cluster of instances.</rdfs:comment>
    <rdfs:domain rdf:resource="http://example.org/onto/class/google_sql_database_instance"/>
    <rdfs:range rdf:resource="http://www.w3.org/2001/XMLSchema#string"/>
  </owl:DatatypeProperty>
  <owl:DatatypeProperty rdf:about="http://example.org/onto/prop/google_sql_database_instance_encryption_key_name">
    <rdfs:label>encryption_key_name</rdfs:label>
    <rdfs:domain rdf:resource="http://example.org/onto/class/google_sql_database_instance"/>
    <rdfs:range rdf:resource="http://www.w3.org/2001/XMLSchema#string"/>
  </owl:DatatypeProperty>
  <owl:DatatypeProperty rdf:about="http://example.org/onto/prop/google_sql_database_instance_final_backup_description">
    <rdfs:label>final_backup_description</rdfs:label>
    <rdfs:comment>The description of final backup if instance enable create final backup during instance deletion.</rdfs:comment>
    <rdfs:domain rdf:resource="http://example.org/onto/class/google_sql_database_instance"/>
    <rdfs:range rdf:resource="http://www.w3.org/2001/XMLSchema#string"/>
  </owl:DatatypeProperty>
  <owl:DatatypeProperty rdf:about="http://example.org/onto/prop/google_sql_database_instance_first_ip_address">
    <rdfs:label>first_ip_address</rdfs:label>
    <rdfs:comment>The first IPv4 address of any type assigned. This is to support accessing the first address in the list in a terraform output when the resource is configured with a count.</rdfs:comment>
    <rdfs:domain rdf:resource="http://example.org/onto/class/google_sql_database_instance"/>
    <rdfs:range rdf:resource="http://www.w3.org/2001/XMLSchema#string"/>
  </owl:DatatypeProperty>
  <owl:DatatypeProperty rdf:about="http://example.org/onto/prop/google_sql_database_instance_id">
    <rdfs:label>id</rdfs:label>
    <rdfs:domain rdf:resource="http://example.org/onto/class/google_sql_database_instance"/>
    <rdfs:range rdf:resource="http://www.w3.org/2001/XMLSchema#string"/>
  </owl:DatatypeProperty>
  <owl:DatatypeProperty rdf:about="http://example.org/onto/prop/google_sql_database_instance_instance_type">
    <rdfs:label>instance_type</rdfs:label>
    <rdfs:comment>The type of the instance. See https://cloud.google.com/sql/docs/mysql/admin-api/rest/v1/instances#SqlInstanceType for supported values.</rdfs:comment>
    <rdfs:domain rdf:resource="http://example.org/onto/class/google_sql_database_instance"/>
    <rdfs:range rdf:resource="http://www.w3.org/2001/XMLSchema#string"/>
  </owl:DatatypeProperty>
  <owl:DatatypeProperty rdf:about="http://example.org/onto/prop/google_sql_database_instance_ip_address">
    <rdfs:label>ip_address</rdfs:label>
    <rdfs:domain rdf:resource="http://example.org/onto/class/google_sql_database_instance"/>
    <rdfs:range rdf:resource="http://www.w3.org/2001/XMLSchema#string"/>
  </owl:DatatypeProperty>
  <owl:DatatypeProperty rdf:about="http://example.org/onto/prop/google_sql_database_instance_maintenance_version">
    <rdfs:label>maintenance_version</rdfs:label>
    <rdfs:comment>Maintenance version.</rdfs:comment>
    <rdfs:domain rdf:resource="http://example.org/onto/class/google_sql_database_instance"/>
    <rdfs:range rdf:resource="http://www.w3.org/2001/XMLSchema#string"/>
  </owl:DatatypeProperty>
  <owl:DatatypeProperty rdf:about="http://example.org/onto/prop/google_sql_database_instance_master_instance_name">
    <rdfs:label>master_instance_name</rdfs:label>
    <rdfs:comment>The name of the instance that will act as the master in the replication setup. Note, this requires the master to have binary_log_enabled set, as well as existing backups.</rdfs:comment>
    <rdfs:domain rdf:resource="http://example.org/onto/class/google_sql_database_instance"/>
    <rdfs:range rdf:resource="http://www.w3.org/2001/XMLSchema#string"/>
  </owl:DatatypeProperty>
  <owl:DatatypeProperty rdf:about="http://example.org/onto/prop/google_sql_database_instance_name">
    <rdfs:label>name</rdfs:label>
    <rdfs:comment>The name of the instance. If the name is left blank, Terraform will randomly generate one when the instance is first created. This is done because after a name is used, it cannot be reused for up to one week.</rdfs:comment>
    <rdfs:domain rdf:resource="http://example.org/onto/class/google_sql_database_instance"/>
    <rdfs:range rdf:resource="http://www.w3.org/2001/XMLSchema#string"/>
  </owl:DatatypeProperty>
  <owl:DatatypeProperty rdf:about="http://example.org/onto/prop/google_sql_database_instance_node_count">
    <rdfs:label>node_count</rdfs:label>
    <rdfs:comment>For a read pool instance, the number of nodes in the read pool.</rdfs:comment>
    <rdfs:domain rdf:resource="http://example.org/onto/class/google_sql_database_instance"/>
    <rdfs:range rdf:resource="http://www.w3.org/2001/XMLSchema#string"/>
  </owl:DatatypeProperty>
  <owl:DatatypeProperty rdf:about="http://example.org/onto/prop/google_sql_database_instance_private_ip_address">
    <rdfs:label>private_ip_address</rdfs:label>
    <rdfs:comment>IPv4 address assigned. This is a workaround for an issue fixed in Terraform 0.12 but also provides a convenient way to access an IP of a specific type without performing filtering in a Terraform config.</rdfs:comment>
    <rdfs:domain rdf:resource="http://example.org/onto/class/google_sql_database_instance"/>
    <rdfs:range rdf:resource="http://www.w3.org/2001/XMLSchema#string"/>
  </owl:DatatypeProperty>
  <owl:DatatypeProperty rdf:about="http://example.org/onto/prop/google_sql_database_instance_project">
    <rdfs:label>project</rdfs:label>
    <rdfs:comment>The ID of the project in which the resource belongs. If it is not provided, the provider project is used.</rdfs:comment>
    <rdfs:domain rdf:resource="http://example.org/onto/class/google_sql_database_instance"/>
    <rdfs:range rdf:resource="http://www.w3.org/2001/XMLSchema#string"/>
  </owl:DatatypeProperty>
  <owl:DatatypeProperty rdf:about="http://example.org/onto/prop/google_sql_database_instance_psc_service_attachment_link">
    <rdfs:label>psc_service_attachment_link</rdfs:label>
    <rdfs:comment>The link to service attachment of PSC instance.</rdfs:comment>
    <rdfs:domain rdf:resource="http://example.org/onto/class/google_sql_database_instance"/>
    <rdfs:range rdf:resource="http://www.w3.org/2001/XMLSchema#string"/>
  </owl:DatatypeProperty>
  <owl:DatatypeProperty rdf:about="http://example.org/onto/prop/google_sql_database_instance_public_ip_address">
    <rdfs:label>public_ip_address</rdfs:label>
    <rdfs:comment>IPv4 address assigned. This is a workaround for an issue fixed in Terraform 0.12 but also provides a convenient way to access an IP of a specific type without performing filtering in a Terraform config.</rdfs:comment>
    <rdfs:domain rdf:resource="http://example.org/onto/class/google_sql_database_instance"/>
    <rdfs:range rdf:resource="http://www.w3.org/2001/XMLSchema#string"/>
  </owl:DatatypeProperty>
  <owl:DatatypeProperty rdf:about="http://example.org/onto/prop/google_sql_database_instance_region">
    <rdfs:label>region</rdfs:label>
    <rdfs:comment>The region the instance will sit in. Note, Cloud SQL is not available in all regions. A valid region must be provided to use this resource. If a region is not provided in the resource definition, the provider region will be used instead, but this will be an apply-time error for instances if the provider region is not supported with Cloud SQL. If you choose not to provide the region argument for this resource, make sure you understand this.</rdfs:comment>
    <rdfs:domain rdf:resource="http://example.org/onto/class/google_sql_database_instance"/>
    <rdfs:range rdf:resource="http://www.w3.org/2001/XMLSchema#string"/>
  </owl:DatatypeProperty>
  <owl:DatatypeProperty rdf:about="http://example.org/onto/prop/google_sql_database_instance_replica_names">
    <rdfs:label>replica_names</rdfs:label>
    <rdfs:comment>The replicas of the instance.</rdfs:comment>
    <rdfs:domain rdf:resource="http://example.org/onto/class/google_sql_database_instance"/>
    <rdfs:range rdf:resource="http://www.w3.org/2001/XMLSchema#string"/>
  </owl:DatatypeProperty>
  <owl:DatatypeProperty rdf:about="http://example.org/onto/prop/google_sql_database_instance_root_password">
    <rdfs:label>root_password</rdfs:label>
    <rdfs:comment>Initial root password. Required for MS SQL Server.</rdfs:comment>
    <rdfs:domain rdf:resource="http://example.org/onto/class/google_sql_database_instance"/>
    <rdfs:range rdf:resource="http://www.w3.org/2001/XMLSchema#string"/>
  </owl:DatatypeProperty>
  <owl:DatatypeProperty rdf:about="http://example.org/onto/prop/google_sql_database_instance_self_link">
    <rdfs:label>self_link</rdfs:label>
    <rdfs:comment>The URI of the created resource.</rdfs:comment>
    <rdfs:domain rdf:resource="http://example.org/onto/class/google_sql_database_instance"/>
    <rdfs:range rdf:resource="http://www.w3.org/2001/XMLSchema#string"/>
  </owl:DatatypeProperty>
  <owl:DatatypeProperty rdf:about="http://example.org/onto/prop/google_sql_database_instance_server_ca_cert">
    <rdfs:label>server_ca_cert</rdfs:label>
    <rdfs:domain rdf:resource="http://example.org/onto/class/google_sql_database_instance"/>
    <rdfs:range rdf:resource="http://www.w3.org/2001/XMLSchema#string"/>
  </owl:DatatypeProperty>
  <owl:DatatypeProperty rdf:about="http://example.org/onto/prop/google_sql_database_instance_service_account_email_address">
    <rdfs:label>service_account_email_address</rdfs:label>
    <rdfs:comment>The service account email address assigned to the instance.</rdfs:comment>
    <rdfs:domain rdf:resource="http://example.org/onto/class/google_sql_database_instance"/>
    <rdfs:range rdf:resource="http://www.w3.org/2001/XMLSchema#string"/>
  </owl:DatatypeProperty>
  <owl:DatatypeProperty rdf:about="http://example.org/onto/prop/google_sql_database_instance_allocated_ip_range">
    <rdfs:label>allocated_ip_range</rdfs:label>
    <rdfs:comment>The name of the allocated ip range for the private ip CloudSQL instance. For example: "google-managed-services-default". If set, the cloned instance ip will be created in the allocated range. The range name must comply with [RFC 1035](https://tools.ietf.org/html/rfc1035). Specifically, the name must be 1-63 characters long and match the regular expression [a-z]([-a-z0-9]*[a-z0-9])?.</rdfs:comment>
    <rdfs:domain rdf:resource="http://example.org/onto/class/google_sql_database_instance"/>
    <rdfs:range rdf:resource="http://www.w3.org/2001/XMLSchema#string"/>
  </owl:DatatypeProperty>
  <owl:DatatypeProperty rdf:about="http://example.org/onto/prop/google_sql_database_instance_database_names">
    <rdfs:label>database_names</rdfs:label>
    <rdfs:comment>(SQL Server only, use with point_in_time) clone only the specified databases from the source instance. Clone all databases if empty.</rdfs:comment>
    <rdfs:domain rdf:resource="http://example.org/onto/class/google_sql_database_instance"/>
    <rdfs:range rdf:resource="http://www.w3.org/2001/XMLSchema#string"/>
  </owl:DatatypeProperty>
  <owl:DatatypeProperty rdf:about="http://example.org/onto/prop/google_sql_database_instance_point_in_time">
    <rdfs:label>point_in_time</rdfs:label>
    <rdfs:comment>The timestamp of the point in time that should be restored.</rdfs:comment>
    <rdfs:domain rdf:resource="http://example.org/onto/class/google_sql_database_instance"/>
    <rdfs:range rdf:resource="http://www.w3.org/2001/XMLSchema#string"/>
  </owl:DatatypeProperty>
  <owl:DatatypeProperty rdf:about="http://example.org/onto/prop/google_sql_database_instance_preferred_zone">
    <rdfs:label>preferred_zone</rdfs:label>
    <rdfs:comment>(Point-in-time recovery for PostgreSQL only) Clone to an instance in the specified zone. If no zone is specified, clone to the same zone as the source instance.</rdfs:comment>
    <rdfs:domain rdf:resource="http://example.org/onto/class/google_sql_database_instance"/>
    <rdfs:range rdf:resource="http://www.w3.org/2001/XMLSchema#string"/>
  </owl:DatatypeProperty>
  <owl:DatatypeProperty rdf:about="http://example.org/onto/prop/google_sql_database_instance_source_instance_deletion_time">
    <rdfs:label>source_instance_deletion_time</rdfs:label>
    <rdfs:comment>The timestamp of when the source instance was deleted for a clone from a deleted instance.</rdfs:comment>
    <rdfs:domain rdf:resource="http://example.org/onto/class/google_sql_database_instance"/>
    <rdfs:range rdf:resource="http://www.w3.org/2001/XMLSchema#string"/>
  </owl:DatatypeProperty>
  <owl:DatatypeProperty rdf:about="http://example.org/onto/prop/google_sql_database_instance_source_instance_name">
    <rdfs:label>source_instance_name</rdfs:label>
    <rdfs:comment>The name of the instance from which the point in time should be restored.</rdfs:comment>
    <rdfs:domain rdf:resource="http://example.org/onto/class/google_sql_database_instance"/>
    <rdfs:range rdf:resource="http://www.w3.org/2001/XMLSchema#string"/>
  </owl:DatatypeProperty>
  <owl:DatatypeProperty rdf:about="http://example.org/onto/prop/google_sql_database_instance_allocated_ip_range">
    <rdfs:label>allocated_ip_range</rdfs:label>
    <rdfs:comment>The name of the allocated IP range for the internal IP Cloud SQL instance. For example: "google-managed-services-default". If you set this, then Cloud SQL creates the IP address for the cloned instance in the allocated range. This range must comply with [RFC 1035](https://tools.ietf.org/html/rfc1035) standards. Specifically, the name must be 1-63 characters long and match the regular expression [a-z]([-a-z0-9]*[a-z0-9])?.</rdfs:comment>
    <rdfs:domain rdf:resource="http://example.org/onto/class/google_sql_database_instance"/>
    <rdfs:range rdf:resource="http://www.w3.org/2001/XMLSchema#string"/>
  </owl:DatatypeProperty>
  <owl:DatatypeProperty rdf:about="http://example.org/onto/prop/google_sql_database_instance_datasource">
    <rdfs:label>datasource</rdfs:label>
    <rdfs:comment>The Google Cloud Backup and Disaster Recovery Datasource URI. For example: "projects/my-project/locations/us-central1/datasources/my-datasource".</rdfs:comment>
    <rdfs:domain rdf:resource="http://example.org/onto/class/google_sql_database_instance"/>
    <rdfs:range rdf:resource="http://www.w3.org/2001/XMLSchema#string"/>
  </owl:DatatypeProperty>
  <owl:DatatypeProperty rdf:about="http://example.org/onto/prop/google_sql_database_instance_point_in_time">
    <rdfs:label>point_in_time</rdfs:label>
    <rdfs:comment>The date and time to which you want to restore the instance.</rdfs:comment>
    <rdfs:domain rdf:resource="http://example.org/onto/class/google_sql_database_instance"/>
    <rdfs:range rdf:resource="http://www.w3.org/2001/XMLSchema#string"/>
  </owl:DatatypeProperty>
  <owl:DatatypeProperty rdf:about="http://example.org/onto/prop/google_sql_database_instance_preferred_zone">
    <rdfs:label>preferred_zone</rdfs:label>
    <rdfs:comment>Point-in-time recovery of an instance to the specified zone. If no zone is specified, then clone to the same primary zone as the source instance.</rdfs:comment>
    <rdfs:domain rdf:resource="http://example.org/onto/class/google_sql_database_instance"/>
    <rdfs:range rdf:resource="http://www.w3.org/2001/XMLSchema#string"/>
  </owl:DatatypeProperty>
  <owl:DatatypeProperty rdf:about="http://example.org/onto/prop/google_sql_database_instance_target_instance">
    <rdfs:label>target_instance</rdfs:label>
    <rdfs:comment>The name of the target instance to restore to.</rdfs:comment>
    <rdfs:domain rdf:resource="http://example.org/onto/class/google_sql_database_instance"/>
    <rdfs:range rdf:resource="http://www.w3.org/2001/XMLSchema#string"/>
  </owl:DatatypeProperty>
  <owl:DatatypeProperty rdf:about="http://example.org/onto/prop/google_sql_database_instance_ca_certificate">
    <rdfs:label>ca_certificate</rdfs:label>
    <rdfs:comment>PEM representation of the trusted CA's x509 certificate.</rdfs:comment>
    <rdfs:domain rdf:resource="http://example.org/onto/class/google_sql_database_instance"/>
    <rdfs:range rdf:resource="http://www.w3.org/2001/XMLSchema#string"/>
  </owl:DatatypeProperty>
  <owl:DatatypeProperty rdf:about="http://example.org/onto/prop/google_sql_database_instance_cascadable_replica">
    <rdfs:label>cascadable_replica</rdfs:label>
    <rdfs:comment>Specifies if a SQL Server replica is a cascadable replica. A cascadable replica is a SQL Server cross region replica that supports replica(s) under it.</rdfs:comment>
    <rdfs:domain rdf:resource="http://example.org/onto/class/google_sql_database_instance"/>
    <rdfs:range rdf:resource="http://www.w3.org/2001/XMLSchema#string"/>
  </owl:DatatypeProperty>
  <owl:DatatypeProperty rdf:about="http://example.org/onto/prop/google_sql_database_instance_client_certificate">
    <rdfs:label>client_certificate</rdfs:label>
    <rdfs:comment>PEM representation of the replica's x509 certificate.</rdfs:comment>
    <rdfs:domain rdf:resource="http://example.org/onto/class/google_sql_database_instance"/>
    <rdfs:range rdf:resource="http://www.w3.org/2001/XMLSchema#string"/>
  </owl:DatatypeProperty>
  <owl:DatatypeProperty rdf:about="http://example.org/onto/prop/google_sql_database_instance_client_key">
    <rdfs:label>client_key</rdfs:label>
    <rdfs:comment>PEM representation of the replica's private key. The corresponding public key in encoded in the client_certificate.</rdfs:comment>
    <rdfs:domain rdf:resource="http://example.org/onto/class/google_sql_database_instance"/>
    <rdfs:range rdf:resource="http://www.w3.org/2001/XMLSchema#string"/>
  </owl:DatatypeProperty>
  <owl:DatatypeProperty rdf:about="http://example.org/onto/prop/google_sql_database_instance_connect_retry_interval">
    <rdfs:label>connect_retry_interval</rdfs:label>
    <rdfs:comment>The number of seconds between connect retries. MySQL's default is 60 seconds.</rdfs:comment>
    <rdfs:domain rdf:resource="http://example.org/onto/class/google_sql_database_instance"/>
    <rdfs:range rdf:resource="http://www.w3.org/2001/XMLSchema#string"/>
  </owl:DatatypeProperty>
  <owl:DatatypeProperty rdf:about="http://example.org/onto/prop/google_sql_database_instance_dump_file_path">
    <rdfs:label>dump_file_path</rdfs:label>
    <rdfs:comment>Path to a SQL file in Google Cloud Storage from which replica instances are created. Format is gs://bucket/filename.</rdfs:comment>
    <rdfs:domain rdf:resource="http://example.org/onto/class/google_sql_database_instance"/>
    <rdfs:range rdf:resource="http://www.w3.org/2001/XMLSchema#string"/>
  </owl:DatatypeProperty>
  <owl:DatatypeProperty rdf:about="http://example.org/onto/prop/google_sql_database_instance_failover_target">
    <rdfs:label>failover_target</rdfs:label>
    <rdfs:comment>Specifies if the replica is the failover target. If the field is set to true the replica will be designated as a failover replica. If the master instance fails, the replica instance will be promoted as the new master instance. Not supported for Postgres</rdfs:comment>
    <rdfs:domain rdf:resource="http://example.org/onto/class/google_sql_database_instance"/>
    <rdfs:range rdf:resource="http://www.w3.org/2001/XMLSchema#string"/>
  </owl:DatatypeProperty>
  <owl:DatatypeProperty rdf:about="http://example.org/onto/prop/google_sql_database_instance_master_heartbeat_period">
    <rdfs:label>master_heartbeat_period</rdfs:label>
    <rdfs:comment>Time in ms between replication heartbeats.</rdfs:comment>
    <rdfs:domain rdf:resource="http://example.org/onto/class/google_sql_database_instance"/>
    <rdfs:range rdf:resource="http://www.w3.org/2001/XMLSchema#string"/>
  </owl:DatatypeProperty>
  <owl:DatatypeProperty rdf:about="http://example.org/onto/prop/google_sql_database_instance_password">
    <rdfs:label>password</rdfs:label>
    <rdfs:comment>Password for the replication connection.</rdfs:comment>
    <rdfs:domain rdf:resource="http://example.org/onto/class/google_sql_database_instance"/>
    <rdfs:range rdf:resource="http://www.w3.org/2001/XMLSchema#string"/>
  </owl:DatatypeProperty>
  <owl:DatatypeProperty rdf:about="http://example.org/onto/prop/google_sql_database_instance_ssl_cipher">
    <rdfs:label>ssl_cipher</rdfs:label>
    <rdfs:comment>Permissible ciphers for use in SSL encryption.</rdfs:comment>
    <rdfs:domain rdf:resource="http://example.org/onto/class/google_sql_database_instance"/>
    <rdfs:range rdf:resource="http://www.w3.org/2001/XMLSchema#string"/>
  </owl:DatatypeProperty>
  <owl:DatatypeProperty rdf:about="http://example.org/onto/prop/google_sql_database_instance_username">
    <rdfs:label>username</rdfs:label>
    <rdfs:comment>Username for replication connection.</rdfs:comment>
    <rdfs:domain rdf:resource="http://example.org/onto/class/google_sql_database_instance"/>
    <rdfs:range rdf:resource="http://www.w3.org/2001/XMLSchema#string"/>
  </owl:DatatypeProperty>
  <owl:DatatypeProperty rdf:about="http://example.org/onto/prop/google_sql_database_instance_verify_server_certificate">
    <rdfs:label>verify_server_certificate</rdfs:label>
    <rdfs:comment>True if the master's common name value is checked during the SSL handshake.</rdfs:comment>
    <rdfs:domain rdf:resource="http://example.org/onto/class/google_sql_database_instance"/>
    <rdfs:range rdf:resource="http://www.w3.org/2001/XMLSchema#string"/>
  </owl:DatatypeProperty>
  <owl:DatatypeProperty rdf:about="http://example.org/onto/prop/google_sql_database_instance_dr_replica">
    <rdfs:label>dr_replica</rdfs:label>
    <rdfs:comment>Read-only field that indicates whether the replica is a DR replica.</rdfs:comment>
    <rdfs:domain rdf:resource="http://example.org/onto/class/google_sql_database_instance"/>
    <rdfs:range rdf:resource="http://www.w3.org/2001/XMLSchema#string"/>
  </owl:DatatypeProperty>
  <owl:DatatypeProperty rdf:about="http://example.org/onto/prop/google_sql_database_instance_failover_dr_replica_name">
    <rdfs:label>failover_dr_replica_name</rdfs:label>
    <rdfs:comment>If the instance is a primary instance, then this field identifies the disaster recovery (DR) replica. The standard format of this field is "your-project:your-instance". You can also set this field to "your-instance", but cloud SQL backend will convert it to the aforementioned standard format.</rdfs:comment>
    <rdfs:domain rdf:resource="http://example.org/onto/class/google_sql_database_instance"/>
    <rdfs:range rdf:resource="http://www.w3.org/2001/XMLSchema#string"/>
  </owl:DatatypeProperty>
  <owl:DatatypeProperty rdf:about="http://example.org/onto/prop/google_sql_database_instance_psa_write_endpoint">
    <rdfs:label>psa_write_endpoint</rdfs:label>
    <rdfs:comment>If set, this field indicates this instance has a private service access (PSA) DNS endpoint that is pointing to the primary instance of the cluster. If this instance is the primary, then the DNS endpoint points to this instance. After a switchover or replica failover operation, this DNS endpoint points to the promoted instance. This is a read-only field, returned to the user as information. This field can exist even if a standalone instance doesn't have a DR replica yet or the DR replica is deleted.</rdfs:comment>
    <rdfs:domain rdf:resource="http://example.org/onto/class/google_sql_database_instance"/>
    <rdfs:range rdf:resource="http://www.w3.org/2001/XMLSchema#string"/>
  </owl:DatatypeProperty>
  <owl:DatatypeProperty rdf:about="http://example.org/onto/prop/google_sql_database_instance_backup_run_id">
    <rdfs:label>backup_run_id</rdfs:label>
    <rdfs:comment>The ID of the backup run to restore from.</rdfs:comment>
    <rdfs:domain rdf:resource="http://example.org/onto/class/google_sql_database_instance"/>
    <rdfs:range rdf:resource="http://www.w3.org/2001/XMLSchema#string"/>
  </owl:DatatypeProperty>
  <owl:DatatypeProperty rdf:about="http://example.org/onto/prop/google_sql_database_instance_instance_id">
    <rdfs:label>instance_id</rdfs:label>
    <rdfs:comment>The ID of the instance that the backup was taken from.</rdfs:comment>
    <rdfs:domain rdf:resource="http://example.org/onto/class/google_sql_database_instance"/>
    <rdfs:range rdf:resource="http://www.w3.org/2001/XMLSchema#string"/>
  </owl:DatatypeProperty>
  <owl:DatatypeProperty rdf:about="http://example.org/onto/prop/google_sql_database_instance_project">
    <rdfs:label>project</rdfs:label>
    <rdfs:comment>The full project ID of the source instance.</rdfs:comment>
    <rdfs:domain rdf:resource="http://example.org/onto/class/google_sql_database_instance"/>
    <rdfs:range rdf:resource="http://www.w3.org/2001/XMLSchema#string"/>
  </owl:DatatypeProperty>
  <owl:DatatypeProperty rdf:about="http://example.org/onto/prop/google_sql_database_instance_activation_policy">
    <rdfs:label>activation_policy</rdfs:label>
    <rdfs:comment>This specifies when the instance should be active. Can be either ALWAYS, NEVER or ON_DEMAND.</rdfs:comment>
    <rdfs:domain rdf:resource="http://example.org/onto/class/google_sql_database_instance"/>
    <rdfs:range rdf:resource="http://www.w3.org/2001/XMLSchema#string"/>
  </owl:DatatypeProperty>
  <owl:DatatypeProperty rdf:about="http://example.org/onto/prop/google_sql_database_instance_availability_type">
    <rdfs:label>availability_type</rdfs:label>
    <rdfs:comment>The availability type of the Cloud SQL instance, high availability
(REGIONAL) or single zone (ZONAL). For all instances, ensure that
settings.backup_configuration.enabled is set to true.
For MySQL instances, ensure that settings.backup_configuration.binary_log_enabled is set to true.
For Postgres instances, ensure that settings.backup_configuration.point_in_time_recovery_enabled
is set to true. Defaults to ZONAL.
For read pool instances, this field is read-only. The availability type is changed by specifying
the number of nodes (node_count).</rdfs:comment>
    <rdfs:domain rdf:resource="http://example.org/onto/class/google_sql_database_instance"/>
    <rdfs:range rdf:resource="http://www.w3.org/2001/XMLSchema#string"/>
  </owl:DatatypeProperty>
  <owl:DatatypeProperty rdf:about="http://example.org/onto/prop/google_sql_database_instance_collation">
    <rdfs:label>collation</rdfs:label>
    <rdfs:comment>The name of server instance collation.</rdfs:comment>
    <rdfs:domain rdf:resource="http://example.org/onto/class/google_sql_database_instance"/>
    <rdfs:range rdf:resource="http://www.w3.org/2001/XMLSchema#string"/>
  </owl:DatatypeProperty>
  <owl:DatatypeProperty rdf:about="http://example.org/onto/prop/google_sql_database_instance_connector_enforcement">
    <rdfs:label>connector_enforcement</rdfs:label>
    <rdfs:comment>Enables the enforcement of Cloud SQL Auth Proxy or Cloud SQL connectors for all the connections. If enabled, all the direct connections are rejected.</rdfs:comment>
    <rdfs:domain rdf:resource="http://example.org/onto/class/google_sql_database_instance"/>
    <rdfs:range rdf:resource="http://www.w3.org/2001/XMLSchema#string"/>
  </owl:DatatypeProperty>
  <owl:DatatypeProperty rdf:about="http://example.org/onto/prop/google_sql_database_instance_deletion_protection_enabled">
    <rdfs:label>deletion_protection_enabled</rdfs:label>
    <rdfs:comment>Configuration to protect against accidental instance deletion.</rdfs:comment>
    <rdfs:domain rdf:resource="http://example.org/onto/class/google_sql_database_instance"/>
    <rdfs:range rdf:resource="http://www.w3.org/2001/XMLSchema#string"/>
  </owl:DatatypeProperty>
  <owl:DatatypeProperty rdf:about="http://example.org/onto/prop/google_sql_database_instance_disk_autoresize">
    <rdfs:label>disk_autoresize</rdfs:label>
    <rdfs:comment>Enables auto-resizing of the storage size. Defaults to true.</rdfs:comment>
    <rdfs:domain rdf:resource="http://example.org/onto/class/google_sql_database_instance"/>
    <rdfs:range rdf:resource="http://www.w3.org/2001/XMLSchema#string"/>
  </owl:DatatypeProperty>
  <owl:DatatypeProperty rdf:about="http://example.org/onto/prop/google_sql_database_instance_disk_autoresize_limit">
    <rdfs:label>disk_autoresize_limit</rdfs:label>
    <rdfs:comment>The maximum size, in GB, to which storage capacity can be automatically increased. The default value is 0, which specifies that there is no limit.</rdfs:comment>
    <rdfs:domain rdf:resource="http://example.org/onto/class/google_sql_database_instance"/>
    <rdfs:range rdf:resource="http://www.w3.org/2001/XMLSchema#string"/>
  </owl:DatatypeProperty>
  <owl:DatatypeProperty rdf:about="http://example.org/onto/prop/google_sql_database_instance_disk_size">
    <rdfs:label>disk_size</rdfs:label>
    <rdfs:comment>The size of data disk, in GB. Size of a running instance cannot be reduced but can be increased. The minimum value is 10GB for PD_SSD, PD_HDD and 20GB for HYPERDISK_BALANCED.</rdfs:comment>
    <rdfs:domain rdf:resource="http://example.org/onto/class/google_sql_database_instance"/>
    <rdfs:range rdf:resource="http://www.w3.org/2001/XMLSchema#string"/>
  </owl:DatatypeProperty>
  <owl:DatatypeProperty rdf:about="http://example.org/onto/prop/google_sql_database_instance_disk_type">
    <rdfs:label>disk_type</rdfs:label>
    <rdfs:comment>The type of supported data disk is tier dependent and can be PD_SSD or PD_HDD or HYPERDISK_BALANCED.</rdfs:comment>
    <rdfs:domain rdf:resource="http://example.org/onto/class/google_sql_database_instance"/>
    <rdfs:range rdf:resource="http://www.w3.org/2001/XMLSchema#string"/>
  </owl:DatatypeProperty>
  <owl:DatatypeProperty rdf:about="http://example.org/onto/prop/google_sql_database_instance_edition">
    <rdfs:label>edition</rdfs:label>
    <rdfs:comment>The edition of the instance, can be ENTERPRISE or ENTERPRISE_PLUS.</rdfs:comment>
    <rdfs:domain rdf:resource="http://example.org/onto/class/google_sql_database_instance"/>
    <rdfs:range rdf:resource="http://www.w3.org/2001/XMLSchema#string"/>
  </owl:DatatypeProperty>
  <owl:DatatypeProperty rdf:about="http://example.org/onto/prop/google_sql_database_instance_effective_availability_type">
    <rdfs:label>effective_availability_type</rdfs:label>
    <rdfs:comment>The availability type of the Cloud SQL instance, high availability
(REGIONAL) or single zone (ZONAL). This field always contains the value that is reported by the
API (for read pools, effective_availability_type may differ from availability_type).</rdfs:comment>
    <rdfs:domain rdf:resource="http://example.org/onto/class/google_sql_database_instance"/>
    <rdfs:range rdf:resource="http://www.w3.org/2001/XMLSchema#string"/>
  </owl:DatatypeProperty>
  <owl:DatatypeProperty rdf:about="http://example.org/onto/prop/google_sql_database_instance_enable_dataplex_integration">
    <rdfs:label>enable_dataplex_integration</rdfs:label>
    <rdfs:comment>Enables Dataplex Integration.</rdfs:comment>
    <rdfs:domain rdf:resource="http://example.org/onto/class/google_sql_database_instance"/>
    <rdfs:range rdf:resource="http://www.w3.org/2001/XMLSchema#string"/>
  </owl:DatatypeProperty>
  <owl:DatatypeProperty rdf:about="http://example.org/onto/prop/google_sql_database_instance_enable_google_ml_integration">
    <rdfs:label>enable_google_ml_integration</rdfs:label>
    <rdfs:comment>Enables Vertex AI Integration.</rdfs:comment>
    <rdfs:domain rdf:resource="http://example.org/onto/class/google_sql_database_instance"/>
    <rdfs:range rdf:resource="http://www.w3.org/2001/XMLSchema#string"/>
  </owl:DatatypeProperty>
  <owl:DatatypeProperty rdf:about="http://example.org/onto/prop/google_sql_database_instance_pricing_plan">
    <rdfs:label>pricing_plan</rdfs:label>
    <rdfs:comment>Pricing plan for this instance, can only be PER_USE.</rdfs:comment>
    <rdfs:domain rdf:resource="http://example.org/onto/class/google_sql_database_instance"/>
    <rdfs:range rdf:resource="http://www.w3.org/2001/XMLSchema#string"/>
  </owl:DatatypeProperty>
  <owl:DatatypeProperty rdf:about="http://example.org/onto/prop/google_sql_database_instance_retain_backups_on_delete">
    <rdfs:label>retain_backups_on_delete</rdfs:label>
    <rdfs:comment>When this parameter is set to true, Cloud SQL retains backups of the instance even after the instance is deleted. The ON_DEMAND backup will be retained until customer deletes the backup or the project. The AUTOMATED backup will be retained based on the backups retention setting.</rdfs:comment>
    <rdfs:domain rdf:resource="http://example.org/onto/class/google_sql_database_instance"/>
    <rdfs:range rdf:resource="http://www.w3.org/2001/XMLSchema#string"/>
  </owl:DatatypeProperty>
  <owl:DatatypeProperty rdf:about="http://example.org/onto/prop/google_sql_database_instance_tier">
    <rdfs:label>tier</rdfs:label>
    <rdfs:comment>The machine type to use. See tiers for more details and supported versions. Postgres supports only shared-core machine types, and custom machine types such as db-custom-2-13312. See the Custom Machine Type Documentation to learn about specifying custom machine types.</rdfs:comment>
    <rdfs:domain rdf:resource="http://example.org/onto/class/google_sql_database_instance"/>
    <rdfs:range rdf:resource="http://www.w3.org/2001/XMLSchema#string"/>
  </owl:DatatypeProperty>
  <owl:DatatypeProperty rdf:about="http://example.org/onto/prop/google_sql_database_instance_time_zone">
    <rdfs:label>time_zone</rdfs:label>
    <rdfs:comment>The time_zone to be used by the database engine (supported only for SQL Server), in SQL Server timezone format.</rdfs:comment>
    <rdfs:domain rdf:resource="http://example.org/onto/class/google_sql_database_instance"/>
    <rdfs:range rdf:resource="http://www.w3.org/2001/XMLSchema#string"/>
  </owl:DatatypeProperty>
  <owl:DatatypeProperty rdf:about="http://example.org/onto/prop/google_sql_database_instance_user_labels">
    <rdfs:label>user_labels</rdfs:label>
    <rdfs:comment>A set of key/value user label pairs to assign to the instance.</rdfs:comment>
    <rdfs:domain rdf:resource="http://example.org/onto/class/google_sql_database_instance"/>
    <rdfs:range rdf:resource="http://www.w3.org/2001/XMLSchema#string"/>
  </owl:DatatypeProperty>
  <owl:DatatypeProperty rdf:about="http://example.org/onto/prop/google_sql_database_instance_version">
    <rdfs:label>version</rdfs:label>
    <rdfs:comment>Used to make sure changes to the settings block are atomic.</rdfs:comment>
    <rdfs:domain rdf:resource="http://example.org/onto/class/google_sql_database_instance"/>
    <rdfs:range rdf:resource="http://www.w3.org/2001/XMLSchema#string"/>
  </owl:DatatypeProperty>
  <owl:DatatypeProperty rdf:about="http://example.org/onto/prop/google_sql_database_instance_domain">
    <rdfs:label>domain</rdfs:label>
    <rdfs:comment>Domain name of the Active Directory for SQL Server (e.g., mydomain.com).</rdfs:comment>
    <rdfs:domain rdf:resource="http://example.org/onto/class/google_sql_database_instance"/>
    <rdfs:range rdf:resource="http://www.w3.org/2001/XMLSchema#string"/>
  </owl:DatatypeProperty>
  <owl:DatatypeProperty rdf:about="http://example.org/onto/prop/google_sql_database_instance_threads_per_core">
    <rdfs:label>threads_per_core</rdfs:label>
    <rdfs:comment>The number of threads per physical core. Can be 1 or 2.</rdfs:comment>
    <rdfs:domain rdf:resource="http://example.org/onto/class/google_sql_database_instance"/>
    <rdfs:range rdf:resource="http://www.w3.org/2001/XMLSchema#string"/>
  </owl:DatatypeProperty>
  <owl:DatatypeProperty rdf:about="http://example.org/onto/prop/google_sql_database_instance_binary_log_enabled">
    <rdfs:label>binary_log_enabled</rdfs:label>
    <rdfs:comment>True if binary logging is enabled. If settings.backup_configuration.enabled is false, this must be as well. Can only be used with MySQL.</rdfs:comment>
    <rdfs:domain rdf:resource="http://example.org/onto/class/google_sql_database_instance"/>
    <rdfs:range rdf:resource="http://www.w3.org/2001/XMLSchema#string"/>
  </owl:DatatypeProperty>
  <owl:DatatypeProperty rdf:about="http://example.org/onto/prop/google_sql_database_instance_enabled">
    <rdfs:label>enabled</rdfs:label>
    <rdfs:comment>True if backup configuration is enabled.</rdfs:comment>
    <rdfs:domain rdf:resource="http://example.org/onto/class/google_sql_database_instance"/>
    <rdfs:range rdf:resource="http://www.w3.org/2001/XMLSchema#string"/>
  </owl:DatatypeProperty>
  <owl:DatatypeProperty rdf:about="http://example.org/onto/prop/google_sql_database_instance_location">
    <rdfs:label>location</rdfs:label>
    <rdfs:comment>Location of the backup configuration.</rdfs:comment>
    <rdfs:domain rdf:resource="http://example.org/onto/class/google_sql_database_instance"/>
    <rdfs:range rdf:resource="http://www.w3.org/2001/XMLSchema#string"/>
  </owl:DatatypeProperty>
  <owl:DatatypeProperty rdf:about="http://example.org/onto/prop/google_sql_database_instance_point_in_time_recovery_enabled">
    <rdfs:label>point_in_time_recovery_enabled</rdfs:label>
    <rdfs:comment>True if Point-in-time recovery is enabled.</rdfs:comment>
    <rdfs:domain rdf:resource="http://example.org/onto/class/google_sql_database_instance"/>
    <rdfs:range rdf:resource="http://www.w3.org/2001/XMLSchema#string"/>
  </owl:DatatypeProperty>
  <owl:DatatypeProperty rdf:about="http://example.org/onto/prop/google_sql_database_instance_start_time">
    <rdfs:label>start_time</rdfs:label>
    <rdfs:comment>HH:MM format time indicating when backup configuration starts.</rdfs:comment>
    <rdfs:domain rdf:resource="http://example.org/onto/class/google_sql_database_instance"/>
    <rdfs:range rdf:resource="http://www.w3.org/2001/XMLSchema#string"/>
  </owl:DatatypeProperty>
  <owl:DatatypeProperty rdf:about="http://example.org/onto/prop/google_sql_database_instance_transaction_log_retention_days">
    <rdfs:label>transaction_log_retention_days</rdfs:label>
    <rdfs:comment>The number of days of transaction logs we retain for point in time restore, from 1-7. (For PostgreSQL Enterprise Plus instances, from 1 to 35.)</rdfs:comment>
    <rdfs:domain rdf:resource="http://example.org/onto/class/google_sql_database_instance"/>
    <rdfs:range rdf:resource="http://www.w3.org/2001/XMLSchema#string"/>
  </owl:DatatypeProperty>
  <owl:DatatypeProperty rdf:about="http://example.org/onto/prop/google_sql_database_instance_retained_backups">
    <rdfs:label>retained_backups</rdfs:label>
    <rdfs:comment>Number of backups to retain.</rdfs:comment>
    <rdfs:domain rdf:resource="http://example.org/onto/class/google_sql_database_instance"/>
    <rdfs:range rdf:resource="http://www.w3.org/2001/XMLSchema#string"/>
  </owl:DatatypeProperty>
  <owl:DatatypeProperty rdf:about="http://example.org/onto/prop/google_sql_database_instance_retention_unit">
    <rdfs:label>retention_unit</rdfs:label>
    <rdfs:comment>The unit that 'retainedBackups' represents. Defaults to COUNT</rdfs:comment>
    <rdfs:domain rdf:resource="http://example.org/onto/class/google_sql_database_instance"/>
    <rdfs:range rdf:resource="http://www.w3.org/2001/XMLSchema#string"/>
  </owl:DatatypeProperty>
  <owl:DatatypeProperty rdf:about="http://example.org/onto/prop/google_sql_database_instance_connection_pooling_enabled">
    <rdfs:label>connection_pooling_enabled</rdfs:label>
    <rdfs:comment>Whether Managed Connection Pool is enabled for this instance.</rdfs:comment>
    <rdfs:domain rdf:resource="http://example.org/onto/class/google_sql_database_instance"/>
    <rdfs:range rdf:resource="http://www.w3.org/2001/XMLSchema#string"/>
  </owl:DatatypeProperty>
  <owl:DatatypeProperty rdf:about="http://example.org/onto/prop/google_sql_database_instance_name">
    <rdfs:label>name</rdfs:label>
    <rdfs:comment>Name of the flag.</rdfs:comment>
    <rdfs:domain rdf:resource="http://example.org/onto/class/google_sql_database_instance"/>
    <rdfs:range rdf:resource="http://www.w3.org/2001/XMLSchema#string"/>
  </owl:DatatypeProperty>
  <owl:DatatypeProperty rdf:about="http://example.org/onto/prop/google_sql_database_instance_value">
    <rdfs:label>value</rdfs:label>
    <rdfs:comment>Value of the flag.</rdfs:comment>
    <rdfs:domain rdf:resource="http://example.org/onto/class/google_sql_database_instance"/>
    <rdfs:range rdf:resource="http://www.w3.org/2001/XMLSchema#string"/>
  </owl:DatatypeProperty>
  <owl:DatatypeProperty rdf:about="http://example.org/onto/prop/google_sql_database_instance_data_cache_enabled">
    <rdfs:label>data_cache_enabled</rdfs:label>
    <rdfs:comment>Whether data cache is enabled for the instance.</rdfs:comment>
    <rdfs:domain rdf:resource="http://example.org/onto/class/google_sql_database_instance"/>
    <rdfs:range rdf:resource="http://www.w3.org/2001/XMLSchema#string"/>
  </owl:DatatypeProperty>
  <owl:DatatypeProperty rdf:about="http://example.org/onto/prop/google_sql_database_instance_name">
    <rdfs:label>name</rdfs:label>
    <rdfs:comment>Name of the flag.</rdfs:comment>
    <rdfs:domain rdf:resource="http://example.org/onto/class/google_sql_database_instance"/>
    <rdfs:range rdf:resource="http://www.w3.org/2001/XMLSchema#string"/>
  </owl:DatatypeProperty>
  <owl:DatatypeProperty rdf:about="http://example.org/onto/prop/google_sql_database_instance_value">
    <rdfs:label>value</rdfs:label>
    <rdfs:comment>Value of the flag.</rdfs:comment>
    <rdfs:domain rdf:resource="http://example.org/onto/class/google_sql_database_instance"/>
    <rdfs:range rdf:resource="http://www.w3.org/2001/XMLSchema#string"/>
  </owl:DatatypeProperty>
  <owl:DatatypeProperty rdf:about="http://example.org/onto/prop/google_sql_database_instance_end_date">
    <rdfs:label>end_date</rdfs:label>
    <rdfs:comment>End date before which maintenance will not take place. The date is in format yyyy-mm-dd i.e., 2020-11-01, or mm-dd, i.e., 11-01</rdfs:comment>
    <rdfs:domain rdf:resource="http://example.org/onto/class/google_sql_database_instance"/>
    <rdfs:range rdf:resource="http://www.w3.org/2001/XMLSchema#string"/>
  </owl:DatatypeProperty>
  <owl:DatatypeProperty rdf:about="http://example.org/onto/prop/google_sql_database_instance_start_date">
    <rdfs:label>start_date</rdfs:label>
    <rdfs:comment>Start date after which maintenance will not take place. The date is in format yyyy-mm-dd i.e., 2020-11-01, or mm-dd, i.e., 11-01</rdfs:comment>
    <rdfs:domain rdf:resource="http://example.org/onto/class/google_sql_database_instance"/>
    <rdfs:range rdf:resource="http://www.w3.org/2001/XMLSchema#string"/>
  </owl:DatatypeProperty>
  <owl:DatatypeProperty rdf:about="http://example.org/onto/prop/google_sql_database_instance_time">
    <rdfs:label>time</rdfs:label>
    <rdfs:comment>Time in UTC when the "deny maintenance period" starts on start_date and ends on end_date. The time is in format: HH:mm:SS, i.e., 00:00:00</rdfs:comment>
    <rdfs:domain rdf:resource="http://example.org/onto/class/google_sql_database_instance"/>
    <rdfs:range rdf:resource="http://www.w3.org/2001/XMLSchema#string"/>
  </owl:DatatypeProperty>
  <owl:DatatypeProperty rdf:about="http://example.org/onto/prop/google_sql_database_instance_enabled">
    <rdfs:label>enabled</rdfs:label>
    <rdfs:comment>When this parameter is set to true, the final backup is enabled for the instance</rdfs:comment>
    <rdfs:domain rdf:resource="http://example.org/onto/class/google_sql_database_instance"/>
    <rdfs:range rdf:resource="http://www.w3.org/2001/XMLSchema#string"/>
  </owl:DatatypeProperty>
  <owl:DatatypeProperty rdf:about="http://example.org/onto/prop/google_sql_database_instance_retention_days">
    <rdfs:label>retention_days</rdfs:label>
    <rdfs:comment>The number of days to retain the final backup after the instance deletion. The valid range is between 1 and 365. For instances managed by BackupDR, the valid range is between 1 day and 99 years. The final backup will be purged at (time_of_instance_deletion + retention_days).</rdfs:comment>
    <rdfs:domain rdf:resource="http://example.org/onto/class/google_sql_database_instance"/>
    <rdfs:range rdf:resource="http://www.w3.org/2001/XMLSchema#string"/>
  </owl:DatatypeProperty>
  <owl:DatatypeProperty rdf:about="http://example.org/onto/prop/google_sql_database_instance_query_insights_enabled">
    <rdfs:label>query_insights_enabled</rdfs:label>
    <rdfs:comment>True if Query Insights feature is enabled.</rdfs:comment>
    <rdfs:domain rdf:resource="http://example.org/onto/class/google_sql_database_instance"/>
    <rdfs:range rdf:resource="http://www.w3.org/2001/XMLSchema#string"/>
  </owl:DatatypeProperty>
  <owl:DatatypeProperty rdf:about="http://example.org/onto/prop/google_sql_database_instance_query_plans_per_minute">
    <rdfs:label>query_plans_per_minute</rdfs:label>
    <rdfs:comment>Number of query execution plans captured by Insights per minute for all queries combined. Between 0 and 20. Default to 5. For Enterprise Plus instances, from 0 to 200.</rdfs:comment>
    <rdfs:domain rdf:resource="http://example.org/onto/class/google_sql_database_instance"/>
    <rdfs:range rdf:resource="http://www.w3.org/2001/XMLSchema#string"/>
  </owl:DatatypeProperty>
  <owl:DatatypeProperty rdf:about="http://example.org/onto/prop/google_sql_database_instance_query_string_length">
    <rdfs:label>query_string_length</rdfs:label>
    <rdfs:comment>Maximum query length stored in bytes. Between 256 and 4500. Default to 1024. For Enterprise Plus instances, from 1 to 1048576.</rdfs:comment>
    <rdfs:domain rdf:resource="http://example.org/onto/class/google_sql_database_instance"/>
    <rdfs:range rdf:resource="http://www.w3.org/2001/XMLSchema#string"/>
  </owl:DatatypeProperty>
  <owl:DatatypeProperty rdf:about="http://example.org/onto/prop/google_sql_database_instance_record_application_tags">
    <rdfs:label>record_application_tags</rdfs:label>
    <rdfs:comment>True if Query Insights will record application tags from query when enabled.</rdfs:comment>
    <rdfs:domain rdf:resource="http://example.org/onto/class/google_sql_database_instance"/>
    <rdfs:range rdf:resource="http://www.w3.org/2001/XMLSchema#string"/>
  </owl:DatatypeProperty>
  <owl:DatatypeProperty rdf:about="http://example.org/onto/prop/google_sql_database_instance_record_client_address">
    <rdfs:label>record_client_address</rdfs:label>
    <rdfs:comment>True if Query Insights will record client address when enabled.</rdfs:comment>
    <rdfs:domain rdf:resource="http://example.org/onto/class/google_sql_database_instance"/>
    <rdfs:range rdf:resource="http://www.w3.org/2001/XMLSchema#string"/>
  </owl:DatatypeProperty>
  <owl:DatatypeProperty rdf:about="http://example.org/onto/prop/google_sql_database_instance_allocated_ip_range">
    <rdfs:label>allocated_ip_range</rdfs:label>
    <rdfs:comment>The name of the allocated ip range for the private ip CloudSQL instance. For example: "google-managed-services-default". If set, the instance ip will be created in the allocated range. The range name must comply with RFC 1035. Specifically, the name must be 1-63 characters long and match the regular expression [a-z]([-a-z0-9]*[a-z0-9])?.</rdfs:comment>
    <rdfs:domain rdf:resource="http://example.org/onto/class/google_sql_database_instance"/>
    <rdfs:range rdf:resource="http://www.w3.org/2001/XMLSchema#string"/>
  </owl:DatatypeProperty>
  <owl:DatatypeProperty rdf:about="http://example.org/onto/prop/google_sql_database_instance_custom_subject_alternative_names">
    <rdfs:label>custom_subject_alternative_names</rdfs:label>
    <rdfs:comment>The custom subject alternative names for an instance with "CUSTOMER_MANAGED_CAS_CA" as the "server_ca_mode".</rdfs:comment>
    <rdfs:domain rdf:resource="http://example.org/onto/class/google_sql_database_instance"/>
    <rdfs:range rdf:resource="http://www.w3.org/2001/XMLSchema#string"/>
  </owl:DatatypeProperty>
  <owl:DatatypeProperty rdf:about="http://example.org/onto/prop/google_sql_database_instance_enable_private_path_for_google_cloud_services">
    <rdfs:label>enable_private_path_for_google_cloud_services</rdfs:label>
    <rdfs:comment>Whether Google Cloud services such as BigQuery are allowed to access data in this Cloud SQL instance over a private IP connection. SQLSERVER database type is not supported.</rdfs:comment>
    <rdfs:domain rdf:resource="http://example.org/onto/class/google_sql_database_instance"/>
    <rdfs:range rdf:resource="http://www.w3.org/2001/XMLSchema#string"/>
  </owl:DatatypeProperty>
  <owl:DatatypeProperty rdf:about="http://example.org/onto/prop/google_sql_database_instance_ipv4_enabled">
    <rdfs:label>ipv4_enabled</rdfs:label>
    <rdfs:comment>Whether this Cloud SQL instance should be assigned a public IPV4 address. At least ipv4_enabled must be enabled or a private_network must be configured.</rdfs:comment>
    <rdfs:domain rdf:resource="http://example.org/onto/class/google_sql_database_instance"/>
    <rdfs:range rdf:resource="http://www.w3.org/2001/XMLSchema#string"/>
  </owl:DatatypeProperty>
  <owl:DatatypeProperty rdf:about="http://example.org/onto/prop/google_sql_database_instance_private_network">
    <rdfs:label>private_network</rdfs:label>
    <rdfs:comment>The VPC network from which the Cloud SQL instance is accessible for private IP. For example, projects/myProject/global/networks/default. Specifying a network enables private IP. At least ipv4_enabled must be enabled or a private_network must be configured. This setting can be updated, but it cannot be removed after it is set.</rdfs:comment>
    <rdfs:domain rdf:resource="http://example.org/onto/class/google_sql_database_instance"/>
    <rdfs:range rdf:resource="http://www.w3.org/2001/XMLSchema#string"/>
  </owl:DatatypeProperty>
  <owl:DatatypeProperty rdf:about="http://example.org/onto/prop/google_sql_database_instance_server_ca_mode">
    <rdfs:label>server_ca_mode</rdfs:label>
    <rdfs:comment>Specify how the server certificate's Certificate Authority is hosted.</rdfs:comment>
    <rdfs:domain rdf:resource="http://example.org/onto/class/google_sql_database_instance"/>
    <rdfs:range rdf:resource="http://www.w3.org/2001/XMLSchema#string"/>
  </owl:DatatypeProperty>
  <owl:DatatypeProperty rdf:about="http://example.org/onto/prop/google_sql_database_instance_server_ca_pool">
    <rdfs:label>server_ca_pool</rdfs:label>
    <rdfs:comment>The resource name of the server CA pool for an instance with "CUSTOMER_MANAGED_CAS_CA" as the "server_ca_mode".</rdfs:comment>
    <rdfs:domain rdf:resource="http://example.org/onto/class/google_sql_database_instance"/>
    <rdfs:range rdf:resource="http://www.w3.org/2001/XMLSchema#string"/>
  </owl:DatatypeProperty>
  <owl:DatatypeProperty rdf:about="http://example.org/onto/prop/google_sql_database_instance_ssl_mode">
    <rdfs:label>ssl_mode</rdfs:label>
    <rdfs:comment>Specify how SSL connection should be enforced in DB connections.</rdfs:comment>
    <rdfs:domain rdf:resource="http://example.org/onto/class/google_sql_database_instance"/>
    <rdfs:range rdf:resource="http://www.w3.org/2001/XMLSchema#string"/>
  </owl:DatatypeProperty>
  <owl:DatatypeProperty rdf:about="http://example.org/onto/prop/google_sql_database_instance_expiration_time">
    <rdfs:label>expiration_time</rdfs:label>
    <rdfs:domain rdf:resource="http://example.org/onto/class/google_sql_database_instance"/>
    <rdfs:range rdf:resource="http://www.w3.org/2001/XMLSchema#string"/>
  </owl:DatatypeProperty>
  <owl:DatatypeProperty rdf:about="http://example.org/onto/prop/google_sql_database_instance_name">
    <rdfs:label>name</rdfs:label>
    <rdfs:domain rdf:resource="http://example.org/onto/class/google_sql_database_instance"/>
    <rdfs:range rdf:resource="http://www.w3.org/2001/XMLSchema#string"/>
  </owl:DatatypeProperty>
  <owl:DatatypeProperty rdf:about="http://example.org/onto/prop/google_sql_database_instance_value">
    <rdfs:label>value</rdfs:label>
    <rdfs:domain rdf:resource="http://example.org/onto/class/google_sql_database_instance"/>
    <rdfs:range rdf:resource="http://www.w3.org/2001/XMLSchema#string"/>
  </owl:DatatypeProperty>
  <owl:DatatypeProperty rdf:about="http://example.org/onto/prop/google_sql_database_instance_allowed_consumer_projects">
    <rdfs:label>allowed_consumer_projects</rdfs:label>
    <rdfs:comment>List of consumer projects that are allow-listed for PSC connections to this instance. This instance can be connected to with PSC from any network in these projects. Each consumer project in this list may be represented by a project number (numeric) or by a project id (alphanumeric).</rdfs:comment>
    <rdfs:domain rdf:resource="http://example.org/onto/class/google_sql_database_instance"/>
    <rdfs:range rdf:resource="http://www.w3.org/2001/XMLSchema#string"/>
  </owl:DatatypeProperty>
  <owl:DatatypeProperty rdf:about="http://example.org/onto/prop/google_sql_database_instance_network_attachment_uri">
    <rdfs:label>network_attachment_uri</rdfs:label>
    <rdfs:comment>Name of network attachment resource used to authorize a producer service to connect a PSC interface to the consumer's VPC. For example: "projects/myProject/regions/myRegion/networkAttachments/myNetworkAttachment". This is required to enable outbound connection on a PSC instance.</rdfs:comment>
    <rdfs:domain rdf:resource="http://example.org/onto/class/google_sql_database_instance"/>
    <rdfs:range rdf:resource="http://www.w3.org/2001/XMLSchema#string"/>
  </owl:DatatypeProperty>
  <owl:DatatypeProperty rdf:about="http://example.org/onto/prop/google_sql_database_instance_psc_enabled">
    <rdfs:label>psc_enabled</rdfs:label>
    <rdfs:comment>Whether PSC connectivity is enabled for this instance.</rdfs:comment>
    <rdfs:domain rdf:resource="http://example.org/onto/class/google_sql_database_instance"/>
    <rdfs:range rdf:resource="http://www.w3.org/2001/XMLSchema#string"/>
  </owl:DatatypeProperty>
  <owl:DatatypeProperty rdf:about="http://example.org/onto/prop/google_sql_database_instance_consumer_network">
    <rdfs:label>consumer_network</rdfs:label>
    <rdfs:comment>The consumer network of this consumer endpoint. This must be a resource path that includes both the host project and the network name. The consumer host project of this network might be different from the consumer service project.</rdfs:comment>
    <rdfs:domain rdf:resource="http://example.org/onto/class/google_sql_database_instance"/>
    <rdfs:range rdf:resource="http://www.w3.org/2001/XMLSchema#string"/>
  </owl:DatatypeProperty>
  <owl:DatatypeProperty rdf:about="http://example.org/onto/prop/google_sql_database_instance_consumer_network_status">
    <rdfs:label>consumer_network_status</rdfs:label>
    <rdfs:comment>The connection policy status of the consumer network.</rdfs:comment>
    <rdfs:domain rdf:resource="http://example.org/onto/class/google_sql_database_instance"/>
    <rdfs:range rdf:resource="http://www.w3.org/2001/XMLSchema#string"/>
  </owl:DatatypeProperty>
  <owl:DatatypeProperty rdf:about="http://example.org/onto/prop/google_sql_database_instance_consumer_service_project_id">
    <rdfs:label>consumer_service_project_id</rdfs:label>
    <rdfs:comment>The project ID of consumer service project of this consumer endpoint.</rdfs:comment>
    <rdfs:domain rdf:resource="http://example.org/onto/class/google_sql_database_instance"/>
    <rdfs:range rdf:resource="http://www.w3.org/2001/XMLSchema#string"/>
  </owl:DatatypeProperty>
  <owl:DatatypeProperty rdf:about="http://example.org/onto/prop/google_sql_database_instance_ip_address">
    <rdfs:label>ip_address</rdfs:label>
    <rdfs:comment>The IP address of the consumer endpoint.</rdfs:comment>
    <rdfs:domain rdf:resource="http://example.org/onto/class/google_sql_database_instance"/>
    <rdfs:range rdf:resource="http://www.w3.org/2001/XMLSchema#string"/>
  </owl:DatatypeProperty>
  <owl:DatatypeProperty rdf:about="http://example.org/onto/prop/google_sql_database_instance_status">
    <rdfs:label>status</rdfs:label>
    <rdfs:comment>The connection status of the consumer endpoint.</rdfs:comment>
    <rdfs:domain rdf:resource="http://example.org/onto/class/google_sql_database_instance"/>
    <rdfs:range rdf:resource="http://www.w3.org/2001/XMLSchema#string"/>
  </owl:DatatypeProperty>
  <owl:DatatypeProperty rdf:about="http://example.org/onto/prop/google_sql_database_instance_follow_gae_application">
    <rdfs:label>follow_gae_application</rdfs:label>
    <rdfs:comment>A Google App Engine application whose zone to remain in. Must be in the same region as this instance.</rdfs:comment>
    <rdfs:domain rdf:resource="http://example.org/onto/class/google_sql_database_instance"/>
    <rdfs:range rdf:resource="http://www.w3.org/2001/XMLSchema#string"/>
  </owl:DatatypeProperty>
  <owl:DatatypeProperty rdf:about="http://example.org/onto/prop/google_sql_database_instance_secondary_zone">
    <rdfs:label>secondary_zone</rdfs:label>
    <rdfs:comment>The preferred Compute Engine zone for the secondary/failover</rdfs:comment>
    <rdfs:domain rdf:resource="http://example.org/onto/class/google_sql_database_instance"/>
    <rdfs:range rdf:resource="http://www.w3.org/2001/XMLSchema#string"/>
  </owl:DatatypeProperty>
  <owl:DatatypeProperty rdf:about="http://example.org/onto/prop/google_sql_database_instance_zone">
    <rdfs:label>zone</rdfs:label>
    <rdfs:comment>The preferred compute engine zone.</rdfs:comment>
    <rdfs:domain rdf:resource="http://example.org/onto/class/google_sql_database_instance"/>
    <rdfs:range rdf:resource="http://www.w3.org/2001/XMLSchema#string"/>
  </owl:DatatypeProperty>
  <owl:DatatypeProperty rdf:about="http://example.org/onto/prop/google_sql_database_instance_day">
    <rdfs:label>day</rdfs:label>
    <rdfs:comment>Day of week (1-7), starting on Monday</rdfs:comment>
    <rdfs:domain rdf:resource="http://example.org/onto/class/google_sql_database_instance"/>
    <rdfs:range rdf:resource="http://www.w3.org/2001/XMLSchema#string"/>
  </owl:DatatypeProperty>
  <owl:DatatypeProperty rdf:about="http://example.org/onto/prop/google_sql_database_instance_hour">
    <rdfs:label>hour</rdfs:label>
    <rdfs:comment>Hour of day (0-23), ignored if day not set</rdfs:comment>
    <rdfs:domain rdf:resource="http://example.org/onto/class/google_sql_database_instance"/>
    <rdfs:range rdf:resource="http://www.w3.org/2001/XMLSchema#string"/>
  </owl:DatatypeProperty>
  <owl:DatatypeProperty rdf:about="http://example.org/onto/prop/google_sql_database_instance_update_track">
    <rdfs:label>update_track</rdfs:label>
    <rdfs:comment>Receive updates after one week (canary) or after two weeks (stable) or after five weeks (week5) of notification.</rdfs:comment>
    <rdfs:domain rdf:resource="http://example.org/onto/class/google_sql_database_instance"/>
    <rdfs:range rdf:resource="http://www.w3.org/2001/XMLSchema#string"/>
  </owl:DatatypeProperty>
  <owl:DatatypeProperty rdf:about="http://example.org/onto/prop/google_sql_database_instance_complexity">
    <rdfs:label>complexity</rdfs:label>
    <rdfs:comment>Password complexity.</rdfs:comment>
    <rdfs:domain rdf:resource="http://example.org/onto/class/google_sql_database_instance"/>
    <rdfs:range rdf:resource="http://www.w3.org/2001/XMLSchema#string"/>
  </owl:DatatypeProperty>
  <owl:DatatypeProperty rdf:about="http://example.org/onto/prop/google_sql_database_instance_disallow_username_substring">
    <rdfs:label>disallow_username_substring</rdfs:label>
    <rdfs:comment>Disallow username as a part of the password.</rdfs:comment>
    <rdfs:domain rdf:resource="http://example.org/onto/class/google_sql_database_instance"/>
    <rdfs:range rdf:resource="http://www.w3.org/2001/XMLSchema#string"/>
  </owl:DatatypeProperty>
  <owl:DatatypeProperty rdf:about="http://example.org/onto/prop/google_sql_database_instance_enable_password_policy">
    <rdfs:label>enable_password_policy</rdfs:label>
    <rdfs:comment>Whether the password policy is enabled or not.</rdfs:comment>
    <rdfs:domain rdf:resource="http://example.org/onto/class/google_sql_database_instance"/>
    <rdfs:range rdf:resource="http://www.w3.org/2001/XMLSchema#string"/>
  </owl:DatatypeProperty>
  <owl:DatatypeProperty rdf:about="http://example.org/onto/prop/google_sql_database_instance_min_length">
    <rdfs:label>min_length</rdfs:label>
    <rdfs:comment>Minimum number of characters allowed.</rdfs:comment>
    <rdfs:domain rdf:resource="http://example.org/onto/class/google_sql_database_instance"/>
    <rdfs:range rdf:resource="http://www.w3.org/2001/XMLSchema#string"/>
  </owl:DatatypeProperty>
  <owl:DatatypeProperty rdf:about="http://example.org/onto/prop/google_sql_database_instance_password_change_interval">
    <rdfs:label>password_change_interval</rdfs:label>
    <rdfs:comment>Minimum interval after which the password can be changed. This flag is only supported for PostgresSQL.</rdfs:comment>
    <rdfs:domain rdf:resource="http://example.org/onto/class/google_sql_database_instance"/>
    <rdfs:range rdf:resource="http://www.w3.org/2001/XMLSchema#string"/>
  </owl:DatatypeProperty>
  <owl:DatatypeProperty rdf:about="http://example.org/onto/prop/google_sql_database_instance_reuse_interval">
    <rdfs:label>reuse_interval</rdfs:label>
    <rdfs:comment>Number of previous passwords that cannot be reused.</rdfs:comment>
    <rdfs:domain rdf:resource="http://example.org/onto/class/google_sql_database_instance"/>
    <rdfs:range rdf:resource="http://www.w3.org/2001/XMLSchema#string"/>
  </owl:DatatypeProperty>
  <owl:DatatypeProperty rdf:about="http://example.org/onto/prop/google_sql_database_instance_bucket">
    <rdfs:label>bucket</rdfs:label>
    <rdfs:comment>The name of the destination bucket (e.g., gs://mybucket).</rdfs:comment>
    <rdfs:domain rdf:resource="http://example.org/onto/class/google_sql_database_instance"/>
    <rdfs:range rdf:resource="http://www.w3.org/2001/XMLSchema#string"/>
  </owl:DatatypeProperty>
  <owl:DatatypeProperty rdf:about="http://example.org/onto/prop/google_sql_database_instance_retention_interval">
    <rdfs:label>retention_interval</rdfs:label>
    <rdfs:comment>How long to keep generated audit files. A duration in seconds with up to nine fractional digits, terminated by 's'. Example: "3.5s"..</rdfs:comment>
    <rdfs:domain rdf:resource="http://example.org/onto/class/google_sql_database_instance"/>
    <rdfs:range rdf:resource="http://www.w3.org/2001/XMLSchema#string"/>
  </owl:DatatypeProperty>
  <owl:DatatypeProperty rdf:about="http://example.org/onto/prop/google_sql_database_instance_upload_interval">
    <rdfs:label>upload_interval</rdfs:label>
    <rdfs:comment>How often to upload generated audit files. A duration in seconds with up to nine fractional digits, terminated by 's'. Example: "3.5s".</rdfs:comment>
    <rdfs:domain rdf:resource="http://example.org/onto/class/google_sql_database_instance"/>
    <rdfs:range rdf:resource="http://www.w3.org/2001/XMLSchema#string"/>
  </owl:DatatypeProperty>
  <owl:DatatypeProperty rdf:about="http://example.org/onto/prop/google_sql_database_instance_create">
    <rdfs:label>create</rdfs:label>
    <rdfs:domain rdf:resource="http://example.org/onto/class/google_sql_database_instance"/>
    <rdfs:range rdf:resource="http://www.w3.org/2001/XMLSchema#string"/>
  </owl:DatatypeProperty>
  <owl:DatatypeProperty rdf:about="http://example.org/onto/prop/google_sql_database_instance_delete">
    <rdfs:label>delete</rdfs:label>
    <rdfs:domain rdf:resource="http://example.org/onto/class/google_sql_database_instance"/>
    <rdfs:range rdf:resource="http://www.w3.org/2001/XMLSchema#string"/>
  </owl:DatatypeProperty>
  <owl:DatatypeProperty rdf:about="http://example.org/onto/prop/google_sql_database_instance_update">
    <rdfs:label>update</rdfs:label>
    <rdfs:domain rdf:resource="http://example.org/onto/class/google_sql_database_instance"/>
    <rdfs:range rdf:resource="http://www.w3.org/2001/XMLSchema#string"/>
  </owl:DatatypeProperty>
</rdf:RDF>
