<?xml version="1.0" encoding="UTF-8"?>
<rdf:RDF
  xmlns:rdf="http://www.w3.org/1999/02/22-rdf-syntax-ns#"
  xmlns:rdfs="http://www.w3.org/2000/01/rdf-schema#"
  xmlns:owl="http://www.w3.org/2002/07/owl#"
  xmlns:xsd="http://www.w3.org/2001/XMLSchema#"
  xml:base="http://example.org/onto/">
  <owl:Class rdf:about="http://example.org/onto/class/google_binary_authorization_policy">
    <rdfs:label>google_binary_authorization_policy</rdfs:label>
    <rdfs:comment>#
#     ***     AUTO GENERATED CODE    ***    Type: MMv1     ***
#
# ----------------------------------------------------------------------------
#
#     This code is generated by Magic Modules using the following:
#
#     Configuration: https:#github.com/GoogleCloudPlatform/magic-modules/tree/main/mmv1/products/binaryauthorization/Policy.yaml
#     Template:      https:#github.com/GoogleCloudPlatform/magic-modules/tree/main/mmv1/templates/terraform/resource.html.markdown.tmpl
#
#     DO NOT EDIT this file directly. Any changes made to this file will be
#     overwritten during the next generation cycle.
#
# ----------------------------------------------------------------------------
subcategory: "Binary Authorization"
description: |-
  A policy for container image binary authorization.
---</rdfs:comment>
  </owl:Class>
  <owl:DatatypeProperty rdf:about="http://example.org/onto/prop/google_binary_authorization_policy_description">
    <rdfs:label>description</rdfs:label>
    <rdfs:comment>A descriptive comment.</rdfs:comment>
    <rdfs:domain rdf:resource="http://example.org/onto/class/google_binary_authorization_policy"/>
    <rdfs:range rdf:resource="http://www.w3.org/2001/XMLSchema#string"/>
  </owl:DatatypeProperty>
  <owl:DatatypeProperty rdf:about="http://example.org/onto/prop/google_binary_authorization_policy_global_policy_evaluation_mode">
    <rdfs:label>global_policy_evaluation_mode</rdfs:label>
    <rdfs:comment>Controls the evaluation of a Google-maintained global admission policy
for common system-level images. Images not covered by the global
policy will be subject to the project admission policy. Possible values: ["ENABLE", "DISABLE"]</rdfs:comment>
    <rdfs:domain rdf:resource="http://example.org/onto/class/google_binary_authorization_policy"/>
    <rdfs:range rdf:resource="http://www.w3.org/2001/XMLSchema#string"/>
  </owl:DatatypeProperty>
  <owl:DatatypeProperty rdf:about="http://example.org/onto/prop/google_binary_authorization_policy_id">
    <rdfs:label>id</rdfs:label>
    <rdfs:domain rdf:resource="http://example.org/onto/class/google_binary_authorization_policy"/>
    <rdfs:range rdf:resource="http://www.w3.org/2001/XMLSchema#string"/>
  </owl:DatatypeProperty>
  <owl:DatatypeProperty rdf:about="http://example.org/onto/prop/google_binary_authorization_policy_project">
    <rdfs:label>project</rdfs:label>
    <rdfs:domain rdf:resource="http://example.org/onto/class/google_binary_authorization_policy"/>
    <rdfs:range rdf:resource="http://www.w3.org/2001/XMLSchema#string"/>
  </owl:DatatypeProperty>
  <owl:DatatypeProperty rdf:about="http://example.org/onto/prop/google_binary_authorization_policy_name_pattern">
    <rdfs:label>name_pattern</rdfs:label>
    <rdfs:comment>An image name pattern to whitelist, in the form
'registry/path/to/image'. This supports a trailing * as a
wildcard, but this is allowed only in text after the registry/
part.</rdfs:comment>
    <rdfs:domain rdf:resource="http://example.org/onto/class/google_binary_authorization_policy"/>
    <rdfs:range rdf:resource="http://www.w3.org/2001/XMLSchema#string"/>
  </owl:DatatypeProperty>
  <owl:DatatypeProperty rdf:about="http://example.org/onto/prop/google_binary_authorization_policy_cluster">
    <rdfs:label>cluster</rdfs:label>
    <rdfs:domain rdf:resource="http://example.org/onto/class/google_binary_authorization_policy"/>
    <rdfs:range rdf:resource="http://www.w3.org/2001/XMLSchema#string"/>
  </owl:DatatypeProperty>
  <owl:DatatypeProperty rdf:about="http://example.org/onto/prop/google_binary_authorization_policy_enforcement_mode">
    <rdfs:label>enforcement_mode</rdfs:label>
    <rdfs:comment>The action when a pod creation is denied by the admission rule. Possible values: ["ENFORCED_BLOCK_AND_AUDIT_LOG", "DRYRUN_AUDIT_LOG_ONLY"]</rdfs:comment>
    <rdfs:domain rdf:resource="http://example.org/onto/class/google_binary_authorization_policy"/>
    <rdfs:range rdf:resource="http://www.w3.org/2001/XMLSchema#string"/>
  </owl:DatatypeProperty>
  <owl:DatatypeProperty rdf:about="http://example.org/onto/prop/google_binary_authorization_policy_evaluation_mode">
    <rdfs:label>evaluation_mode</rdfs:label>
    <rdfs:comment>How this admission rule will be evaluated. Possible values: ["ALWAYS_ALLOW", "REQUIRE_ATTESTATION", "ALWAYS_DENY"]</rdfs:comment>
    <rdfs:domain rdf:resource="http://example.org/onto/class/google_binary_authorization_policy"/>
    <rdfs:range rdf:resource="http://www.w3.org/2001/XMLSchema#string"/>
  </owl:DatatypeProperty>
  <owl:DatatypeProperty rdf:about="http://example.org/onto/prop/google_binary_authorization_policy_require_attestations_by">
    <rdfs:label>require_attestations_by</rdfs:label>
    <rdfs:comment>The resource names of the attestors that must attest to a
container image. If the attestor is in a different project from the
policy, it should be specified in the format 'projects/*/attestors/*'.
Each attestor must exist before a policy can reference it. To add an
attestor to a policy the principal issuing the policy change
request must be able to read the attestor resource.

Note: this field must be non-empty when the evaluation_mode field
specifies REQUIRE_ATTESTATION, otherwise it must be empty.</rdfs:comment>
    <rdfs:domain rdf:resource="http://example.org/onto/class/google_binary_authorization_policy"/>
    <rdfs:range rdf:resource="http://www.w3.org/2001/XMLSchema#string"/>
  </owl:DatatypeProperty>
  <owl:DatatypeProperty rdf:about="http://example.org/onto/prop/google_binary_authorization_policy_enforcement_mode">
    <rdfs:label>enforcement_mode</rdfs:label>
    <rdfs:comment>The action when a pod creation is denied by the admission rule. Possible values: ["ENFORCED_BLOCK_AND_AUDIT_LOG", "DRYRUN_AUDIT_LOG_ONLY"]</rdfs:comment>
    <rdfs:domain rdf:resource="http://example.org/onto/class/google_binary_authorization_policy"/>
    <rdfs:range rdf:resource="http://www.w3.org/2001/XMLSchema#string"/>
  </owl:DatatypeProperty>
  <owl:DatatypeProperty rdf:about="http://example.org/onto/prop/google_binary_authorization_policy_evaluation_mode">
    <rdfs:label>evaluation_mode</rdfs:label>
    <rdfs:comment>How this admission rule will be evaluated. Possible values: ["ALWAYS_ALLOW", "REQUIRE_ATTESTATION", "ALWAYS_DENY"]</rdfs:comment>
    <rdfs:domain rdf:resource="http://example.org/onto/class/google_binary_authorization_policy"/>
    <rdfs:range rdf:resource="http://www.w3.org/2001/XMLSchema#string"/>
  </owl:DatatypeProperty>
  <owl:DatatypeProperty rdf:about="http://example.org/onto/prop/google_binary_authorization_policy_require_attestations_by">
    <rdfs:label>require_attestations_by</rdfs:label>
    <rdfs:comment>The resource names of the attestors that must attest to a
container image. If the attestor is in a different project from the
policy, it should be specified in the format 'projects/*/attestors/*'.
Each attestor must exist before a policy can reference it. To add an
attestor to a policy the principal issuing the policy change
request must be able to read the attestor resource.

Note: this field must be non-empty when the evaluation_mode field
specifies REQUIRE_ATTESTATION, otherwise it must be empty.</rdfs:comment>
    <rdfs:domain rdf:resource="http://example.org/onto/class/google_binary_authorization_policy"/>
    <rdfs:range rdf:resource="http://www.w3.org/2001/XMLSchema#string"/>
  </owl:DatatypeProperty>
  <owl:DatatypeProperty rdf:about="http://example.org/onto/prop/google_binary_authorization_policy_create">
    <rdfs:label>create</rdfs:label>
    <rdfs:domain rdf:resource="http://example.org/onto/class/google_binary_authorization_policy"/>
    <rdfs:range rdf:resource="http://www.w3.org/2001/XMLSchema#string"/>
  </owl:DatatypeProperty>
  <owl:DatatypeProperty rdf:about="http://example.org/onto/prop/google_binary_authorization_policy_delete">
    <rdfs:label>delete</rdfs:label>
    <rdfs:domain rdf:resource="http://example.org/onto/class/google_binary_authorization_policy"/>
    <rdfs:range rdf:resource="http://www.w3.org/2001/XMLSchema#string"/>
  </owl:DatatypeProperty>
  <owl:DatatypeProperty rdf:about="http://example.org/onto/prop/google_binary_authorization_policy_update">
    <rdfs:label>update</rdfs:label>
    <rdfs:domain rdf:resource="http://example.org/onto/class/google_binary_authorization_policy"/>
    <rdfs:range rdf:resource="http://www.w3.org/2001/XMLSchema#string"/>
  </owl:DatatypeProperty>
</rdf:RDF>
