<?xml version="1.0" encoding="UTF-8"?>
<rdf:RDF
  xmlns:rdf="http://www.w3.org/1999/02/22-rdf-syntax-ns#"
  xmlns:rdfs="http://www.w3.org/2000/01/rdf-schema#"
  xmlns:owl="http://www.w3.org/2002/07/owl#"
  xmlns:xsd="http://www.w3.org/2001/XMLSchema#"
  xml:base="http://example.org/onto/">
  <owl:Class rdf:about="http://example.org/onto/class/google_managed_kafka_connect_cluster">
    <rdfs:label>google_managed_kafka_connect_cluster</rdfs:label>
    <rdfs:comment>#
#     ***     AUTO GENERATED CODE    ***    Type: MMv1     ***
#
# ----------------------------------------------------------------------------
#
#     This code is generated by Magic Modules using the following:
#
#     Configuration: https:#github.com/GoogleCloudPlatform/magic-modules/tree/main/mmv1/products/managedkafka/ConnectCluster.yaml
#     Template:      https:#github.com/GoogleCloudPlatform/magic-modules/tree/main/mmv1/templates/terraform/resource.html.markdown.tmpl
#
#     DO NOT EDIT this file directly. Any changes made to this file will be
#     overwritten during the next generation cycle.
#
# ----------------------------------------------------------------------------
subcategory: "Managed Kafka"
description: |-
  A Managed Service for Kafka Connect cluster.
---</rdfs:comment>
  </owl:Class>
  <owl:DatatypeProperty rdf:about="http://example.org/onto/prop/google_managed_kafka_connect_cluster_connect_cluster_id">
    <rdfs:label>connect_cluster_id</rdfs:label>
    <rdfs:comment>The ID to use for the Connect Cluster, which will become the final component of the connect cluster's name. This value is structured like: 'my-connect-cluster-id'.</rdfs:comment>
    <rdfs:domain rdf:resource="http://example.org/onto/class/google_managed_kafka_connect_cluster"/>
    <rdfs:range rdf:resource="http://www.w3.org/2001/XMLSchema#string"/>
  </owl:DatatypeProperty>
  <owl:DatatypeProperty rdf:about="http://example.org/onto/prop/google_managed_kafka_connect_cluster_create_time">
    <rdfs:label>create_time</rdfs:label>
    <rdfs:comment>The time when the cluster was created.</rdfs:comment>
    <rdfs:domain rdf:resource="http://example.org/onto/class/google_managed_kafka_connect_cluster"/>
    <rdfs:range rdf:resource="http://www.w3.org/2001/XMLSchema#string"/>
  </owl:DatatypeProperty>
  <owl:DatatypeProperty rdf:about="http://example.org/onto/prop/google_managed_kafka_connect_cluster_effective_labels">
    <rdfs:label>effective_labels</rdfs:label>
    <rdfs:comment>All of labels (key/value pairs) present on the resource in GCP, including the labels configured through Terraform, other clients and services.</rdfs:comment>
    <rdfs:domain rdf:resource="http://example.org/onto/class/google_managed_kafka_connect_cluster"/>
    <rdfs:range rdf:resource="http://www.w3.org/2001/XMLSchema#string"/>
  </owl:DatatypeProperty>
  <owl:DatatypeProperty rdf:about="http://example.org/onto/prop/google_managed_kafka_connect_cluster_id">
    <rdfs:label>id</rdfs:label>
    <rdfs:domain rdf:resource="http://example.org/onto/class/google_managed_kafka_connect_cluster"/>
    <rdfs:range rdf:resource="http://www.w3.org/2001/XMLSchema#string"/>
  </owl:DatatypeProperty>
  <owl:DatatypeProperty rdf:about="http://example.org/onto/prop/google_managed_kafka_connect_cluster_kafka_cluster">
    <rdfs:label>kafka_cluster</rdfs:label>
    <rdfs:comment>The name of the Kafka cluster this Kafka Connect cluster is attached to. Structured like: 'projects/PROJECT_ID/locations/LOCATION/clusters/CLUSTER_ID'.</rdfs:comment>
    <rdfs:domain rdf:resource="http://example.org/onto/class/google_managed_kafka_connect_cluster"/>
    <rdfs:range rdf:resource="http://www.w3.org/2001/XMLSchema#string"/>
  </owl:DatatypeProperty>
  <owl:DatatypeProperty rdf:about="http://example.org/onto/prop/google_managed_kafka_connect_cluster_labels">
    <rdfs:label>labels</rdfs:label>
    <rdfs:comment>List of label KEY=VALUE pairs to add. Keys must start with a lowercase character and contain only hyphens (-), underscores ( ), lowercase characters, and numbers. Values must contain only hyphens (-), underscores ( ), lowercase characters, and numbers.

**Note**: This field is non-authoritative, and will only manage the labels present in your configuration.
Please refer to the field 'effective_labels' for all of the labels present on the resource.</rdfs:comment>
    <rdfs:domain rdf:resource="http://example.org/onto/class/google_managed_kafka_connect_cluster"/>
    <rdfs:range rdf:resource="http://www.w3.org/2001/XMLSchema#string"/>
  </owl:DatatypeProperty>
  <owl:DatatypeProperty rdf:about="http://example.org/onto/prop/google_managed_kafka_connect_cluster_location">
    <rdfs:label>location</rdfs:label>
    <rdfs:comment>ID of the location of the Kafka Connect resource. See https://cloud.google.com/managed-kafka/docs/locations for a list of supported locations.</rdfs:comment>
    <rdfs:domain rdf:resource="http://example.org/onto/class/google_managed_kafka_connect_cluster"/>
    <rdfs:range rdf:resource="http://www.w3.org/2001/XMLSchema#string"/>
  </owl:DatatypeProperty>
  <owl:DatatypeProperty rdf:about="http://example.org/onto/prop/google_managed_kafka_connect_cluster_name">
    <rdfs:label>name</rdfs:label>
    <rdfs:comment>The name of the connect cluster. Structured like: 'projects/PROJECT_ID/locations/LOCATION/connectClusters/CONNECT_CLUSTER_ID'.</rdfs:comment>
    <rdfs:domain rdf:resource="http://example.org/onto/class/google_managed_kafka_connect_cluster"/>
    <rdfs:range rdf:resource="http://www.w3.org/2001/XMLSchema#string"/>
  </owl:DatatypeProperty>
  <owl:DatatypeProperty rdf:about="http://example.org/onto/prop/google_managed_kafka_connect_cluster_project">
    <rdfs:label>project</rdfs:label>
    <rdfs:domain rdf:resource="http://example.org/onto/class/google_managed_kafka_connect_cluster"/>
    <rdfs:range rdf:resource="http://www.w3.org/2001/XMLSchema#string"/>
  </owl:DatatypeProperty>
  <owl:DatatypeProperty rdf:about="http://example.org/onto/prop/google_managed_kafka_connect_cluster_state">
    <rdfs:label>state</rdfs:label>
    <rdfs:comment>The current state of the connect cluster. Possible values: 'STATE_UNSPECIFIED', 'CREATING', 'ACTIVE', 'DELETING'.</rdfs:comment>
    <rdfs:domain rdf:resource="http://example.org/onto/class/google_managed_kafka_connect_cluster"/>
    <rdfs:range rdf:resource="http://www.w3.org/2001/XMLSchema#string"/>
  </owl:DatatypeProperty>
  <owl:DatatypeProperty rdf:about="http://example.org/onto/prop/google_managed_kafka_connect_cluster_terraform_labels">
    <rdfs:label>terraform_labels</rdfs:label>
    <rdfs:comment>The combination of labels configured directly on the resource
 and default labels configured on the provider.</rdfs:comment>
    <rdfs:domain rdf:resource="http://example.org/onto/class/google_managed_kafka_connect_cluster"/>
    <rdfs:range rdf:resource="http://www.w3.org/2001/XMLSchema#string"/>
  </owl:DatatypeProperty>
  <owl:DatatypeProperty rdf:about="http://example.org/onto/prop/google_managed_kafka_connect_cluster_update_time">
    <rdfs:label>update_time</rdfs:label>
    <rdfs:comment>The time when the cluster was last updated.</rdfs:comment>
    <rdfs:domain rdf:resource="http://example.org/onto/class/google_managed_kafka_connect_cluster"/>
    <rdfs:range rdf:resource="http://www.w3.org/2001/XMLSchema#string"/>
  </owl:DatatypeProperty>
  <owl:DatatypeProperty rdf:about="http://example.org/onto/prop/google_managed_kafka_connect_cluster_memory_bytes">
    <rdfs:label>memory_bytes</rdfs:label>
    <rdfs:comment>The memory to provision for the cluster in bytes. The CPU:memory ratio (vCPU:GiB) must be between 1:1 and 1:8. Minimum: 3221225472 (3 GiB).</rdfs:comment>
    <rdfs:domain rdf:resource="http://example.org/onto/class/google_managed_kafka_connect_cluster"/>
    <rdfs:range rdf:resource="http://www.w3.org/2001/XMLSchema#string"/>
  </owl:DatatypeProperty>
  <owl:DatatypeProperty rdf:about="http://example.org/onto/prop/google_managed_kafka_connect_cluster_vcpu_count">
    <rdfs:label>vcpu_count</rdfs:label>
    <rdfs:comment>The number of vCPUs to provision for the cluster. The minimum is 3.</rdfs:comment>
    <rdfs:domain rdf:resource="http://example.org/onto/class/google_managed_kafka_connect_cluster"/>
    <rdfs:range rdf:resource="http://www.w3.org/2001/XMLSchema#string"/>
  </owl:DatatypeProperty>
  <owl:DatatypeProperty rdf:about="http://example.org/onto/prop/google_managed_kafka_connect_cluster_additional_subnets">
    <rdfs:label>additional_subnets</rdfs:label>
    <rdfs:comment>Additional subnets may be specified. They may be in another region, but must be in the same VPC network. The Connect workers can communicate with network endpoints in either the primary or additional subnets.</rdfs:comment>
    <rdfs:domain rdf:resource="http://example.org/onto/class/google_managed_kafka_connect_cluster"/>
    <rdfs:range rdf:resource="http://www.w3.org/2001/XMLSchema#string"/>
  </owl:DatatypeProperty>
  <owl:DatatypeProperty rdf:about="http://example.org/onto/prop/google_managed_kafka_connect_cluster_dns_domain_names">
    <rdfs:label>dns_domain_names</rdfs:label>
    <rdfs:comment>Additional DNS domain names from the subnet's network to be made visible to the Connect Cluster. When using MirrorMaker2, it's necessary to add the bootstrap address's dns domain name of the target cluster to make it visible to the connector. For example: my-kafka-cluster.us-central1.managedkafka.my-project.cloud.goog</rdfs:comment>
    <rdfs:domain rdf:resource="http://example.org/onto/class/google_managed_kafka_connect_cluster"/>
    <rdfs:range rdf:resource="http://www.w3.org/2001/XMLSchema#string"/>
  </owl:DatatypeProperty>
  <owl:DatatypeProperty rdf:about="http://example.org/onto/prop/google_managed_kafka_connect_cluster_primary_subnet">
    <rdfs:label>primary_subnet</rdfs:label>
    <rdfs:comment>VPC subnet to make available to the Kafka Connect cluster. Structured like: projects/{project}/regions/{region}/subnetworks/{subnet_id}. It is used to create a Private Service Connect (PSC) interface for the Kafka Connect workers. It must be located in the same region as the Kafka Connect cluster. The CIDR range of the subnet must be within the IPv4 address ranges for private networks, as specified in RFC 1918. The primary subnet CIDR range must have a minimum size of /22 (1024 addresses).</rdfs:comment>
    <rdfs:domain rdf:resource="http://example.org/onto/class/google_managed_kafka_connect_cluster"/>
    <rdfs:range rdf:resource="http://www.w3.org/2001/XMLSchema#string"/>
  </owl:DatatypeProperty>
  <owl:DatatypeProperty rdf:about="http://example.org/onto/prop/google_managed_kafka_connect_cluster_create">
    <rdfs:label>create</rdfs:label>
    <rdfs:domain rdf:resource="http://example.org/onto/class/google_managed_kafka_connect_cluster"/>
    <rdfs:range rdf:resource="http://www.w3.org/2001/XMLSchema#string"/>
  </owl:DatatypeProperty>
  <owl:DatatypeProperty rdf:about="http://example.org/onto/prop/google_managed_kafka_connect_cluster_delete">
    <rdfs:label>delete</rdfs:label>
    <rdfs:domain rdf:resource="http://example.org/onto/class/google_managed_kafka_connect_cluster"/>
    <rdfs:range rdf:resource="http://www.w3.org/2001/XMLSchema#string"/>
  </owl:DatatypeProperty>
  <owl:DatatypeProperty rdf:about="http://example.org/onto/prop/google_managed_kafka_connect_cluster_update">
    <rdfs:label>update</rdfs:label>
    <rdfs:domain rdf:resource="http://example.org/onto/class/google_managed_kafka_connect_cluster"/>
    <rdfs:range rdf:resource="http://www.w3.org/2001/XMLSchema#string"/>
  </owl:DatatypeProperty>
</rdf:RDF>
