<?xml version="1.0" encoding="UTF-8"?>
<rdf:RDF
  xmlns:rdf="http://www.w3.org/1999/02/22-rdf-syntax-ns#"
  xmlns:rdfs="http://www.w3.org/2000/01/rdf-schema#"
  xmlns:owl="http://www.w3.org/2002/07/owl#"
  xmlns:xsd="http://www.w3.org/2001/XMLSchema#"
  xml:base="http://example.org/onto/">
  <owl:Class rdf:about="http://example.org/onto/class/google_compute_address">
    <rdfs:label>google_compute_address</rdfs:label>
    <rdfs:comment>#
#     ***     AUTO GENERATED CODE    ***    Type: MMv1     ***
#
# ----------------------------------------------------------------------------
#
#     This code is generated by Magic Modules using the following:
#
#     Configuration: https:#github.com/GoogleCloudPlatform/magic-modules/tree/main/mmv1/products/compute/Address.yaml
#     Template:      https:#github.com/GoogleCloudPlatform/magic-modules/tree/main/mmv1/templates/terraform/resource.html.markdown.tmpl
#
#     DO NOT EDIT this file directly. Any changes made to this file will be
#     overwritten during the next generation cycle.
#
# ----------------------------------------------------------------------------
subcategory: "Compute Engine"
description: |-
  Represents an Address resource.
---</rdfs:comment>
  </owl:Class>
  <owl:DatatypeProperty rdf:about="http://example.org/onto/prop/google_compute_address_address">
    <rdfs:label>address</rdfs:label>
    <rdfs:comment>The static external IP address represented by this resource.
The IP address must be inside the specified subnetwork,
if any. Set by the API if undefined.</rdfs:comment>
    <rdfs:domain rdf:resource="http://example.org/onto/class/google_compute_address"/>
    <rdfs:range rdf:resource="http://www.w3.org/2001/XMLSchema#string"/>
  </owl:DatatypeProperty>
  <owl:DatatypeProperty rdf:about="http://example.org/onto/prop/google_compute_address_address_type">
    <rdfs:label>address_type</rdfs:label>
    <rdfs:comment>The type of address to reserve.
Note: if you set this argument's value as 'INTERNAL' you need to leave the 'network_tier' argument unset in that resource block. Default value: "EXTERNAL" Possible values: ["INTERNAL", "EXTERNAL"]</rdfs:comment>
    <rdfs:domain rdf:resource="http://example.org/onto/class/google_compute_address"/>
    <rdfs:range rdf:resource="http://www.w3.org/2001/XMLSchema#string"/>
  </owl:DatatypeProperty>
  <owl:DatatypeProperty rdf:about="http://example.org/onto/prop/google_compute_address_creation_timestamp">
    <rdfs:label>creation_timestamp</rdfs:label>
    <rdfs:comment>Creation timestamp in RFC3339 text format.</rdfs:comment>
    <rdfs:domain rdf:resource="http://example.org/onto/class/google_compute_address"/>
    <rdfs:range rdf:resource="http://www.w3.org/2001/XMLSchema#string"/>
  </owl:DatatypeProperty>
  <owl:DatatypeProperty rdf:about="http://example.org/onto/prop/google_compute_address_description">
    <rdfs:label>description</rdfs:label>
    <rdfs:comment>An optional description of this resource.</rdfs:comment>
    <rdfs:domain rdf:resource="http://example.org/onto/class/google_compute_address"/>
    <rdfs:range rdf:resource="http://www.w3.org/2001/XMLSchema#string"/>
  </owl:DatatypeProperty>
  <owl:DatatypeProperty rdf:about="http://example.org/onto/prop/google_compute_address_effective_labels">
    <rdfs:label>effective_labels</rdfs:label>
    <rdfs:comment>All of labels (key/value pairs) present on the resource in GCP, including the labels configured through Terraform, other clients and services.</rdfs:comment>
    <rdfs:domain rdf:resource="http://example.org/onto/class/google_compute_address"/>
    <rdfs:range rdf:resource="http://www.w3.org/2001/XMLSchema#string"/>
  </owl:DatatypeProperty>
  <owl:DatatypeProperty rdf:about="http://example.org/onto/prop/google_compute_address_id">
    <rdfs:label>id</rdfs:label>
    <rdfs:domain rdf:resource="http://example.org/onto/class/google_compute_address"/>
    <rdfs:range rdf:resource="http://www.w3.org/2001/XMLSchema#string"/>
  </owl:DatatypeProperty>
  <owl:DatatypeProperty rdf:about="http://example.org/onto/prop/google_compute_address_ip_version">
    <rdfs:label>ip_version</rdfs:label>
    <rdfs:comment>The IP Version that will be used by this address. The default value is 'IPV4'. Possible values: ["IPV4", "IPV6"]</rdfs:comment>
    <rdfs:domain rdf:resource="http://example.org/onto/class/google_compute_address"/>
    <rdfs:range rdf:resource="http://www.w3.org/2001/XMLSchema#string"/>
  </owl:DatatypeProperty>
  <owl:DatatypeProperty rdf:about="http://example.org/onto/prop/google_compute_address_ipv6_endpoint_type">
    <rdfs:label>ipv6_endpoint_type</rdfs:label>
    <rdfs:comment>The endpoint type of this address, which should be VM or NETLB. This is
used for deciding which type of endpoint this address can be used after
the external IPv6 address reservation. Possible values: ["VM", "NETLB"]</rdfs:comment>
    <rdfs:domain rdf:resource="http://example.org/onto/class/google_compute_address"/>
    <rdfs:range rdf:resource="http://www.w3.org/2001/XMLSchema#string"/>
  </owl:DatatypeProperty>
  <owl:DatatypeProperty rdf:about="http://example.org/onto/prop/google_compute_address_label_fingerprint">
    <rdfs:label>label_fingerprint</rdfs:label>
    <rdfs:comment>The fingerprint used for optimistic locking of this resource.  Used
internally during updates.</rdfs:comment>
    <rdfs:domain rdf:resource="http://example.org/onto/class/google_compute_address"/>
    <rdfs:range rdf:resource="http://www.w3.org/2001/XMLSchema#string"/>
  </owl:DatatypeProperty>
  <owl:DatatypeProperty rdf:about="http://example.org/onto/prop/google_compute_address_labels">
    <rdfs:label>labels</rdfs:label>
    <rdfs:comment>Labels to apply to this address.  A list of key->value pairs.


**Note**: This field is non-authoritative, and will only manage the labels present in your configuration.
Please refer to the field 'effective_labels' for all of the labels present on the resource.</rdfs:comment>
    <rdfs:domain rdf:resource="http://example.org/onto/class/google_compute_address"/>
    <rdfs:range rdf:resource="http://www.w3.org/2001/XMLSchema#string"/>
  </owl:DatatypeProperty>
  <owl:DatatypeProperty rdf:about="http://example.org/onto/prop/google_compute_address_name">
    <rdfs:label>name</rdfs:label>
    <rdfs:comment>Name of the resource. The name must be 1-63 characters long, and
comply with RFC1035. Specifically, the name must be 1-63 characters
long and match the regular expression '[a-z]([-a-z0-9]*[a-z0-9])?'
which means the first character must be a lowercase letter, and all
following characters must be a dash, lowercase letter, or digit,
except the last character, which cannot be a dash.</rdfs:comment>
    <rdfs:domain rdf:resource="http://example.org/onto/class/google_compute_address"/>
    <rdfs:range rdf:resource="http://www.w3.org/2001/XMLSchema#string"/>
  </owl:DatatypeProperty>
  <owl:DatatypeProperty rdf:about="http://example.org/onto/prop/google_compute_address_network">
    <rdfs:label>network</rdfs:label>
    <rdfs:comment>The URL of the network in which to reserve the address. This field
can only be used with INTERNAL type with the VPC_PEERING and
IPSEC_INTERCONNECT purposes.</rdfs:comment>
    <rdfs:domain rdf:resource="http://example.org/onto/class/google_compute_address"/>
    <rdfs:range rdf:resource="http://www.w3.org/2001/XMLSchema#string"/>
  </owl:DatatypeProperty>
  <owl:DatatypeProperty rdf:about="http://example.org/onto/prop/google_compute_address_network_tier">
    <rdfs:label>network_tier</rdfs:label>
    <rdfs:comment>The networking tier used for configuring this address. If this field is not
specified, it is assumed to be PREMIUM.
This argument should not be used when configuring Internal addresses, because [network tier cannot be set for internal traffic; it's always Premium](https://cloud.google.com/network-tiers/docs/overview). Possible values: ["PREMIUM", "STANDARD"]</rdfs:comment>
    <rdfs:domain rdf:resource="http://example.org/onto/class/google_compute_address"/>
    <rdfs:range rdf:resource="http://www.w3.org/2001/XMLSchema#string"/>
  </owl:DatatypeProperty>
  <owl:DatatypeProperty rdf:about="http://example.org/onto/prop/google_compute_address_prefix_length">
    <rdfs:label>prefix_length</rdfs:label>
    <rdfs:comment>The prefix length if the resource represents an IP range.</rdfs:comment>
    <rdfs:domain rdf:resource="http://example.org/onto/class/google_compute_address"/>
    <rdfs:range rdf:resource="http://www.w3.org/2001/XMLSchema#string"/>
  </owl:DatatypeProperty>
  <owl:DatatypeProperty rdf:about="http://example.org/onto/prop/google_compute_address_project">
    <rdfs:label>project</rdfs:label>
    <rdfs:domain rdf:resource="http://example.org/onto/class/google_compute_address"/>
    <rdfs:range rdf:resource="http://www.w3.org/2001/XMLSchema#string"/>
  </owl:DatatypeProperty>
  <owl:DatatypeProperty rdf:about="http://example.org/onto/prop/google_compute_address_purpose">
    <rdfs:label>purpose</rdfs:label>
    <rdfs:comment>The purpose of this resource, which can be one of the following values.

* GCE_ENDPOINT for addresses that are used by VM instances, alias IP
ranges, load balancers, and similar resources.

* SHARED_LOADBALANCER_VIP for an address that can be used by multiple
internal load balancers.

* VPC_PEERING for addresses that are reserved for VPC peer networks.

* IPSEC_INTERCONNECT for addresses created from a private IP range that
are reserved for a VLAN attachment in an HA VPN over Cloud Interconnect
configuration. These addresses are regional resources.

* PRIVATE_SERVICE_CONNECT for a private network address that is used to
configure Private Service Connect. Only global internal addresses can use
this purpose.

This should only be set when using an Internal address.</rdfs:comment>
    <rdfs:domain rdf:resource="http://example.org/onto/class/google_compute_address"/>
    <rdfs:range rdf:resource="http://www.w3.org/2001/XMLSchema#string"/>
  </owl:DatatypeProperty>
  <owl:DatatypeProperty rdf:about="http://example.org/onto/prop/google_compute_address_region">
    <rdfs:label>region</rdfs:label>
    <rdfs:comment>The Region in which the created address should reside.
If it is not provided, the provider region is used.</rdfs:comment>
    <rdfs:domain rdf:resource="http://example.org/onto/class/google_compute_address"/>
    <rdfs:range rdf:resource="http://www.w3.org/2001/XMLSchema#string"/>
  </owl:DatatypeProperty>
  <owl:DatatypeProperty rdf:about="http://example.org/onto/prop/google_compute_address_self_link">
    <rdfs:label>self_link</rdfs:label>
    <rdfs:domain rdf:resource="http://example.org/onto/class/google_compute_address"/>
    <rdfs:range rdf:resource="http://www.w3.org/2001/XMLSchema#string"/>
  </owl:DatatypeProperty>
  <owl:DatatypeProperty rdf:about="http://example.org/onto/prop/google_compute_address_subnetwork">
    <rdfs:label>subnetwork</rdfs:label>
    <rdfs:comment>The URL of the subnetwork in which to reserve the address. If an IP
address is specified, it must be within the subnetwork's IP range.
This field can only be used with INTERNAL type with
GCE_ENDPOINT/DNS_RESOLVER purposes.</rdfs:comment>
    <rdfs:domain rdf:resource="http://example.org/onto/class/google_compute_address"/>
    <rdfs:range rdf:resource="http://www.w3.org/2001/XMLSchema#string"/>
  </owl:DatatypeProperty>
  <owl:DatatypeProperty rdf:about="http://example.org/onto/prop/google_compute_address_terraform_labels">
    <rdfs:label>terraform_labels</rdfs:label>
    <rdfs:comment>The combination of labels configured directly on the resource
 and default labels configured on the provider.</rdfs:comment>
    <rdfs:domain rdf:resource="http://example.org/onto/class/google_compute_address"/>
    <rdfs:range rdf:resource="http://www.w3.org/2001/XMLSchema#string"/>
  </owl:DatatypeProperty>
  <owl:DatatypeProperty rdf:about="http://example.org/onto/prop/google_compute_address_users">
    <rdfs:label>users</rdfs:label>
    <rdfs:comment>The URLs of the resources that are using this address.</rdfs:comment>
    <rdfs:domain rdf:resource="http://example.org/onto/class/google_compute_address"/>
    <rdfs:range rdf:resource="http://www.w3.org/2001/XMLSchema#string"/>
  </owl:DatatypeProperty>
  <owl:DatatypeProperty rdf:about="http://example.org/onto/prop/google_compute_address_create">
    <rdfs:label>create</rdfs:label>
    <rdfs:domain rdf:resource="http://example.org/onto/class/google_compute_address"/>
    <rdfs:range rdf:resource="http://www.w3.org/2001/XMLSchema#string"/>
  </owl:DatatypeProperty>
  <owl:DatatypeProperty rdf:about="http://example.org/onto/prop/google_compute_address_delete">
    <rdfs:label>delete</rdfs:label>
    <rdfs:domain rdf:resource="http://example.org/onto/class/google_compute_address"/>
    <rdfs:range rdf:resource="http://www.w3.org/2001/XMLSchema#string"/>
  </owl:DatatypeProperty>
  <owl:DatatypeProperty rdf:about="http://example.org/onto/prop/google_compute_address_update">
    <rdfs:label>update</rdfs:label>
    <rdfs:domain rdf:resource="http://example.org/onto/class/google_compute_address"/>
    <rdfs:range rdf:resource="http://www.w3.org/2001/XMLSchema#string"/>
  </owl:DatatypeProperty>
</rdf:RDF>
