<?xml version="1.0" encoding="UTF-8"?>
<rdf:RDF
  xmlns:rdf="http://www.w3.org/1999/02/22-rdf-syntax-ns#"
  xmlns:rdfs="http://www.w3.org/2000/01/rdf-schema#"
  xmlns:owl="http://www.w3.org/2002/07/owl#"
  xmlns:xsd="http://www.w3.org/2001/XMLSchema#"
  xml:base="http://example.org/onto/">
  <owl:Class rdf:about="http://example.org/onto/class/google_iam_folders_policy_binding">
    <rdfs:label>google_iam_folders_policy_binding</rdfs:label>
    <rdfs:comment>#
#     ***     AUTO GENERATED CODE    ***    Type: MMv1     ***
#
# ----------------------------------------------------------------------------
#
#     This code is generated by Magic Modules using the following:
#
#     Configuration: https:#github.com/GoogleCloudPlatform/magic-modules/tree/main/mmv1/products/iam3/FoldersPolicyBinding.yaml
#     Template:      https:#github.com/GoogleCloudPlatform/magic-modules/tree/main/mmv1/templates/terraform/resource.html.markdown.tmpl
#
#     DO NOT EDIT this file directly. Any changes made to this file will be
#     overwritten during the next generation cycle.
#
# ----------------------------------------------------------------------------
subcategory: "Cloud IAM"
description: |-
  A policy binding to a folder.
---</rdfs:comment>
  </owl:Class>
  <owl:DatatypeProperty rdf:about="http://example.org/onto/prop/google_iam_folders_policy_binding_annotations">
    <rdfs:label>annotations</rdfs:label>
    <rdfs:comment>Optional. User defined annotations. See https://google.aip.dev/148#annotations for more details such as format and size limitations


**Note**: This field is non-authoritative, and will only manage the annotations present in your configuration.
Please refer to the field 'effective_annotations' for all of the annotations present on the resource.</rdfs:comment>
    <rdfs:domain rdf:resource="http://example.org/onto/class/google_iam_folders_policy_binding"/>
    <rdfs:range rdf:resource="http://www.w3.org/2001/XMLSchema#string"/>
  </owl:DatatypeProperty>
  <owl:DatatypeProperty rdf:about="http://example.org/onto/prop/google_iam_folders_policy_binding_create_time">
    <rdfs:label>create_time</rdfs:label>
    <rdfs:comment>Output only. The time when the policy binding was created.</rdfs:comment>
    <rdfs:domain rdf:resource="http://example.org/onto/class/google_iam_folders_policy_binding"/>
    <rdfs:range rdf:resource="http://www.w3.org/2001/XMLSchema#string"/>
  </owl:DatatypeProperty>
  <owl:DatatypeProperty rdf:about="http://example.org/onto/prop/google_iam_folders_policy_binding_display_name">
    <rdfs:label>display_name</rdfs:label>
    <rdfs:comment>Optional. The description of the policy binding. Must be less than or equal to 63 characters.</rdfs:comment>
    <rdfs:domain rdf:resource="http://example.org/onto/class/google_iam_folders_policy_binding"/>
    <rdfs:range rdf:resource="http://www.w3.org/2001/XMLSchema#string"/>
  </owl:DatatypeProperty>
  <owl:DatatypeProperty rdf:about="http://example.org/onto/prop/google_iam_folders_policy_binding_effective_annotations">
    <rdfs:label>effective_annotations</rdfs:label>
    <rdfs:comment>All of annotations (key/value pairs) present on the resource in GCP, including the annotations configured through Terraform, other clients and services.</rdfs:comment>
    <rdfs:domain rdf:resource="http://example.org/onto/class/google_iam_folders_policy_binding"/>
    <rdfs:range rdf:resource="http://www.w3.org/2001/XMLSchema#string"/>
  </owl:DatatypeProperty>
  <owl:DatatypeProperty rdf:about="http://example.org/onto/prop/google_iam_folders_policy_binding_etag">
    <rdfs:label>etag</rdfs:label>
    <rdfs:comment>Optional. The etag for the policy binding. If this is provided on update, it must match the server's etag.</rdfs:comment>
    <rdfs:domain rdf:resource="http://example.org/onto/class/google_iam_folders_policy_binding"/>
    <rdfs:range rdf:resource="http://www.w3.org/2001/XMLSchema#string"/>
  </owl:DatatypeProperty>
  <owl:DatatypeProperty rdf:about="http://example.org/onto/prop/google_iam_folders_policy_binding_folder">
    <rdfs:label>folder</rdfs:label>
    <rdfs:comment>The parent folder for the PolicyBinding.</rdfs:comment>
    <rdfs:domain rdf:resource="http://example.org/onto/class/google_iam_folders_policy_binding"/>
    <rdfs:range rdf:resource="http://www.w3.org/2001/XMLSchema#string"/>
  </owl:DatatypeProperty>
  <owl:DatatypeProperty rdf:about="http://example.org/onto/prop/google_iam_folders_policy_binding_id">
    <rdfs:label>id</rdfs:label>
    <rdfs:domain rdf:resource="http://example.org/onto/class/google_iam_folders_policy_binding"/>
    <rdfs:range rdf:resource="http://www.w3.org/2001/XMLSchema#string"/>
  </owl:DatatypeProperty>
  <owl:DatatypeProperty rdf:about="http://example.org/onto/prop/google_iam_folders_policy_binding_location">
    <rdfs:label>location</rdfs:label>
    <rdfs:comment>The location of the PolicyBinding.</rdfs:comment>
    <rdfs:domain rdf:resource="http://example.org/onto/class/google_iam_folders_policy_binding"/>
    <rdfs:range rdf:resource="http://www.w3.org/2001/XMLSchema#string"/>
  </owl:DatatypeProperty>
  <owl:DatatypeProperty rdf:about="http://example.org/onto/prop/google_iam_folders_policy_binding_name">
    <rdfs:label>name</rdfs:label>
    <rdfs:comment>The name of the policy binding in the format '{binding_parent/locations/{location}/policyBindings/{policy_binding_id}'</rdfs:comment>
    <rdfs:domain rdf:resource="http://example.org/onto/class/google_iam_folders_policy_binding"/>
    <rdfs:range rdf:resource="http://www.w3.org/2001/XMLSchema#string"/>
  </owl:DatatypeProperty>
  <owl:DatatypeProperty rdf:about="http://example.org/onto/prop/google_iam_folders_policy_binding_policy">
    <rdfs:label>policy</rdfs:label>
    <rdfs:comment>Required. Immutable. The resource name of the policy to be bound. The binding parent and policy must belong to the same Organization (or Project).</rdfs:comment>
    <rdfs:domain rdf:resource="http://example.org/onto/class/google_iam_folders_policy_binding"/>
    <rdfs:range rdf:resource="http://www.w3.org/2001/XMLSchema#string"/>
  </owl:DatatypeProperty>
  <owl:DatatypeProperty rdf:about="http://example.org/onto/prop/google_iam_folders_policy_binding_policy_binding_id">
    <rdfs:label>policy_binding_id</rdfs:label>
    <rdfs:comment>The Policy Binding ID.</rdfs:comment>
    <rdfs:domain rdf:resource="http://example.org/onto/class/google_iam_folders_policy_binding"/>
    <rdfs:range rdf:resource="http://www.w3.org/2001/XMLSchema#string"/>
  </owl:DatatypeProperty>
  <owl:DatatypeProperty rdf:about="http://example.org/onto/prop/google_iam_folders_policy_binding_policy_kind">
    <rdfs:label>policy_kind</rdfs:label>
    <rdfs:comment>Immutable. The kind of the policy to attach in this binding. This
field must be one of the following:  - Left empty (will be automatically set
to the policy kind) - The input policy kind   Possible values:  POLICY_KIND_UNSPECIFIED PRINCIPAL_ACCESS_BOUNDARY ACCESS</rdfs:comment>
    <rdfs:domain rdf:resource="http://example.org/onto/class/google_iam_folders_policy_binding"/>
    <rdfs:range rdf:resource="http://www.w3.org/2001/XMLSchema#string"/>
  </owl:DatatypeProperty>
  <owl:DatatypeProperty rdf:about="http://example.org/onto/prop/google_iam_folders_policy_binding_policy_uid">
    <rdfs:label>policy_uid</rdfs:label>
    <rdfs:comment>Output only. The globally unique ID of the policy to be bound.</rdfs:comment>
    <rdfs:domain rdf:resource="http://example.org/onto/class/google_iam_folders_policy_binding"/>
    <rdfs:range rdf:resource="http://www.w3.org/2001/XMLSchema#string"/>
  </owl:DatatypeProperty>
  <owl:DatatypeProperty rdf:about="http://example.org/onto/prop/google_iam_folders_policy_binding_uid">
    <rdfs:label>uid</rdfs:label>
    <rdfs:comment>Output only. The globally unique ID of the policy binding. Assigned when the policy binding is created.</rdfs:comment>
    <rdfs:domain rdf:resource="http://example.org/onto/class/google_iam_folders_policy_binding"/>
    <rdfs:range rdf:resource="http://www.w3.org/2001/XMLSchema#string"/>
  </owl:DatatypeProperty>
  <owl:DatatypeProperty rdf:about="http://example.org/onto/prop/google_iam_folders_policy_binding_update_time">
    <rdfs:label>update_time</rdfs:label>
    <rdfs:comment>Output only. The time when the policy binding was most recently updated.</rdfs:comment>
    <rdfs:domain rdf:resource="http://example.org/onto/class/google_iam_folders_policy_binding"/>
    <rdfs:range rdf:resource="http://www.w3.org/2001/XMLSchema#string"/>
  </owl:DatatypeProperty>
  <owl:DatatypeProperty rdf:about="http://example.org/onto/prop/google_iam_folders_policy_binding_description">
    <rdfs:label>description</rdfs:label>
    <rdfs:comment>Optional. Description of the expression. This is a longer text which describes the expression, e.g. when hovered over it in a UI.</rdfs:comment>
    <rdfs:domain rdf:resource="http://example.org/onto/class/google_iam_folders_policy_binding"/>
    <rdfs:range rdf:resource="http://www.w3.org/2001/XMLSchema#string"/>
  </owl:DatatypeProperty>
  <owl:DatatypeProperty rdf:about="http://example.org/onto/prop/google_iam_folders_policy_binding_expression">
    <rdfs:label>expression</rdfs:label>
    <rdfs:comment>Textual representation of an expression in Common Expression Language syntax.</rdfs:comment>
    <rdfs:domain rdf:resource="http://example.org/onto/class/google_iam_folders_policy_binding"/>
    <rdfs:range rdf:resource="http://www.w3.org/2001/XMLSchema#string"/>
  </owl:DatatypeProperty>
  <owl:DatatypeProperty rdf:about="http://example.org/onto/prop/google_iam_folders_policy_binding_location">
    <rdfs:label>location</rdfs:label>
    <rdfs:comment>Optional. String indicating the location of the expression for error reporting, e.g. a file name and a position in the file.</rdfs:comment>
    <rdfs:domain rdf:resource="http://example.org/onto/class/google_iam_folders_policy_binding"/>
    <rdfs:range rdf:resource="http://www.w3.org/2001/XMLSchema#string"/>
  </owl:DatatypeProperty>
  <owl:DatatypeProperty rdf:about="http://example.org/onto/prop/google_iam_folders_policy_binding_title">
    <rdfs:label>title</rdfs:label>
    <rdfs:comment>Optional. Title for the expression, i.e. a short string describing its purpose. This can be used e.g. in UIs which allow to enter the expression.</rdfs:comment>
    <rdfs:domain rdf:resource="http://example.org/onto/class/google_iam_folders_policy_binding"/>
    <rdfs:range rdf:resource="http://www.w3.org/2001/XMLSchema#string"/>
  </owl:DatatypeProperty>
  <owl:DatatypeProperty rdf:about="http://example.org/onto/prop/google_iam_folders_policy_binding_principal_set">
    <rdfs:label>principal_set</rdfs:label>
    <rdfs:comment>Required. Immutable. Full Resource Name of the principal set used for principal access boundary policy bindings.
Examples for each one of the following supported principal set types:
* Folder: '//cloudresourcemanager.googleapis.com/folders/FOLDER_ID'
It must be parent by the policy binding's parent (the folder).</rdfs:comment>
    <rdfs:domain rdf:resource="http://example.org/onto/class/google_iam_folders_policy_binding"/>
    <rdfs:range rdf:resource="http://www.w3.org/2001/XMLSchema#string"/>
  </owl:DatatypeProperty>
  <owl:DatatypeProperty rdf:about="http://example.org/onto/prop/google_iam_folders_policy_binding_create">
    <rdfs:label>create</rdfs:label>
    <rdfs:domain rdf:resource="http://example.org/onto/class/google_iam_folders_policy_binding"/>
    <rdfs:range rdf:resource="http://www.w3.org/2001/XMLSchema#string"/>
  </owl:DatatypeProperty>
  <owl:DatatypeProperty rdf:about="http://example.org/onto/prop/google_iam_folders_policy_binding_delete">
    <rdfs:label>delete</rdfs:label>
    <rdfs:domain rdf:resource="http://example.org/onto/class/google_iam_folders_policy_binding"/>
    <rdfs:range rdf:resource="http://www.w3.org/2001/XMLSchema#string"/>
  </owl:DatatypeProperty>
  <owl:DatatypeProperty rdf:about="http://example.org/onto/prop/google_iam_folders_policy_binding_update">
    <rdfs:label>update</rdfs:label>
    <rdfs:domain rdf:resource="http://example.org/onto/class/google_iam_folders_policy_binding"/>
    <rdfs:range rdf:resource="http://www.w3.org/2001/XMLSchema#string"/>
  </owl:DatatypeProperty>
</rdf:RDF>
