<?xml version="1.0" encoding="UTF-8"?>
<rdf:RDF
  xmlns:rdf="http://www.w3.org/1999/02/22-rdf-syntax-ns#"
  xmlns:rdfs="http://www.w3.org/2000/01/rdf-schema#"
  xmlns:owl="http://www.w3.org/2002/07/owl#"
  xmlns:xsd="http://www.w3.org/2001/XMLSchema#"
  xml:base="http://example.org/onto/">
  <owl:Class rdf:about="http://example.org/onto/class/google_iam_workforce_pool">
    <rdfs:label>google_iam_workforce_pool</rdfs:label>
    <rdfs:comment>#
#     ***     AUTO GENERATED CODE    ***    Type: MMv1     ***
#
# ----------------------------------------------------------------------------
#
#     This code is generated by Magic Modules using the following:
#
#     Configuration: https:#github.com/GoogleCloudPlatform/magic-modules/tree/main/mmv1/products/iamworkforcepool/WorkforcePool.yaml
#     Template:      https:#github.com/GoogleCloudPlatform/magic-modules/tree/main/mmv1/templates/terraform/resource.html.markdown.tmpl
#
#     DO NOT EDIT this file directly. Any changes made to this file will be
#     overwritten during the next generation cycle.
#
# ----------------------------------------------------------------------------
subcategory: "Cloud IAM"
description: |-
  Represents a collection of external workforces.
---</rdfs:comment>
  </owl:Class>
  <owl:DatatypeProperty rdf:about="http://example.org/onto/prop/google_iam_workforce_pool_description">
    <rdfs:label>description</rdfs:label>
    <rdfs:comment>A user-specified description of the pool. Cannot exceed 256 characters.</rdfs:comment>
    <rdfs:domain rdf:resource="http://example.org/onto/class/google_iam_workforce_pool"/>
    <rdfs:range rdf:resource="http://www.w3.org/2001/XMLSchema#string"/>
  </owl:DatatypeProperty>
  <owl:DatatypeProperty rdf:about="http://example.org/onto/prop/google_iam_workforce_pool_disabled">
    <rdfs:label>disabled</rdfs:label>
    <rdfs:comment>Whether the pool is disabled. You cannot use a disabled pool to exchange tokens,
or use existing tokens to access resources. If the pool is re-enabled, existing tokens grant access again.</rdfs:comment>
    <rdfs:domain rdf:resource="http://example.org/onto/class/google_iam_workforce_pool"/>
    <rdfs:range rdf:resource="http://www.w3.org/2001/XMLSchema#string"/>
  </owl:DatatypeProperty>
  <owl:DatatypeProperty rdf:about="http://example.org/onto/prop/google_iam_workforce_pool_display_name">
    <rdfs:label>display_name</rdfs:label>
    <rdfs:comment>A user-specified display name of the pool in Google Cloud Console. Cannot exceed 32 characters.</rdfs:comment>
    <rdfs:domain rdf:resource="http://example.org/onto/class/google_iam_workforce_pool"/>
    <rdfs:range rdf:resource="http://www.w3.org/2001/XMLSchema#string"/>
  </owl:DatatypeProperty>
  <owl:DatatypeProperty rdf:about="http://example.org/onto/prop/google_iam_workforce_pool_id">
    <rdfs:label>id</rdfs:label>
    <rdfs:domain rdf:resource="http://example.org/onto/class/google_iam_workforce_pool"/>
    <rdfs:range rdf:resource="http://www.w3.org/2001/XMLSchema#string"/>
  </owl:DatatypeProperty>
  <owl:DatatypeProperty rdf:about="http://example.org/onto/prop/google_iam_workforce_pool_location">
    <rdfs:label>location</rdfs:label>
    <rdfs:comment>The location for the resource.</rdfs:comment>
    <rdfs:domain rdf:resource="http://example.org/onto/class/google_iam_workforce_pool"/>
    <rdfs:range rdf:resource="http://www.w3.org/2001/XMLSchema#string"/>
  </owl:DatatypeProperty>
  <owl:DatatypeProperty rdf:about="http://example.org/onto/prop/google_iam_workforce_pool_name">
    <rdfs:label>name</rdfs:label>
    <rdfs:comment>Output only. The resource name of the pool.
Format: 'locations/{location}/workforcePools/{workforcePoolId}'</rdfs:comment>
    <rdfs:domain rdf:resource="http://example.org/onto/class/google_iam_workforce_pool"/>
    <rdfs:range rdf:resource="http://www.w3.org/2001/XMLSchema#string"/>
  </owl:DatatypeProperty>
  <owl:DatatypeProperty rdf:about="http://example.org/onto/prop/google_iam_workforce_pool_parent">
    <rdfs:label>parent</rdfs:label>
    <rdfs:comment>Immutable. The resource name of the parent. Format: 'organizations/{org-id}'.</rdfs:comment>
    <rdfs:domain rdf:resource="http://example.org/onto/class/google_iam_workforce_pool"/>
    <rdfs:range rdf:resource="http://www.w3.org/2001/XMLSchema#string"/>
  </owl:DatatypeProperty>
  <owl:DatatypeProperty rdf:about="http://example.org/onto/prop/google_iam_workforce_pool_session_duration">
    <rdfs:label>session_duration</rdfs:label>
    <rdfs:comment>Duration that the Google Cloud access tokens, console sign-in sessions,
and 'gcloud' sign-in sessions from this pool are valid.
Must be greater than 15 minutes (900s) and less than 12 hours (43200s).
If 'sessionDuration' is not configured, minted credentials have a default duration of one hour (3600s).
A duration in seconds with up to nine fractional digits, ending with ''s''. Example: "'3.5s'".</rdfs:comment>
    <rdfs:domain rdf:resource="http://example.org/onto/class/google_iam_workforce_pool"/>
    <rdfs:range rdf:resource="http://www.w3.org/2001/XMLSchema#string"/>
  </owl:DatatypeProperty>
  <owl:DatatypeProperty rdf:about="http://example.org/onto/prop/google_iam_workforce_pool_state">
    <rdfs:label>state</rdfs:label>
    <rdfs:comment>Output only. The state of the pool.
 * STATE_UNSPECIFIED: State unspecified.
 * ACTIVE: The pool is active, and may be used in Google Cloud policies.
 * DELETED: The pool is soft-deleted. Soft-deleted pools are permanently deleted
   after approximately 30 days. You can restore a soft-deleted pool using
   [workforcePools.undelete](https://cloud.google.com/iam/docs/reference/rest/v1/locations.workforcePools/undelete#google.iam.admin.v1.WorkforcePools.UndeleteWorkforcePool).
   You cannot reuse the ID of a soft-deleted pool until it is permanently deleted.
   While a pool is deleted, you cannot use it to exchange tokens, or use
   existing tokens to access resources. If the pool is undeleted, existing
   tokens grant access again.</rdfs:comment>
    <rdfs:domain rdf:resource="http://example.org/onto/class/google_iam_workforce_pool"/>
    <rdfs:range rdf:resource="http://www.w3.org/2001/XMLSchema#string"/>
  </owl:DatatypeProperty>
  <owl:DatatypeProperty rdf:about="http://example.org/onto/prop/google_iam_workforce_pool_workforce_pool_id">
    <rdfs:label>workforce_pool_id</rdfs:label>
    <rdfs:comment>The name of the pool. The ID must be a globally unique string of 6 to 63 lowercase letters,
digits, or hyphens. It must start with a letter, and cannot have a trailing hyphen.
The prefix 'gcp-' is reserved for use by Google, and may not be specified.</rdfs:comment>
    <rdfs:domain rdf:resource="http://example.org/onto/class/google_iam_workforce_pool"/>
    <rdfs:range rdf:resource="http://www.w3.org/2001/XMLSchema#string"/>
  </owl:DatatypeProperty>
  <owl:DatatypeProperty rdf:about="http://example.org/onto/prop/google_iam_workforce_pool_disable_programmatic_signin">
    <rdfs:label>disable_programmatic_signin</rdfs:label>
    <rdfs:comment>Disable programmatic sign-in by disabling token issue via the Security Token API endpoint.
See [Security Token Service API](https://cloud.google.com/iam/docs/reference/sts/rest).</rdfs:comment>
    <rdfs:domain rdf:resource="http://example.org/onto/class/google_iam_workforce_pool"/>
    <rdfs:range rdf:resource="http://www.w3.org/2001/XMLSchema#string"/>
  </owl:DatatypeProperty>
  <owl:DatatypeProperty rdf:about="http://example.org/onto/prop/google_iam_workforce_pool_domain">
    <rdfs:label>domain</rdfs:label>
    <rdfs:comment>Domain name of the service.
Example: console.cloud.google</rdfs:comment>
    <rdfs:domain rdf:resource="http://example.org/onto/class/google_iam_workforce_pool"/>
    <rdfs:range rdf:resource="http://www.w3.org/2001/XMLSchema#string"/>
  </owl:DatatypeProperty>
  <owl:DatatypeProperty rdf:about="http://example.org/onto/prop/google_iam_workforce_pool_create">
    <rdfs:label>create</rdfs:label>
    <rdfs:domain rdf:resource="http://example.org/onto/class/google_iam_workforce_pool"/>
    <rdfs:range rdf:resource="http://www.w3.org/2001/XMLSchema#string"/>
  </owl:DatatypeProperty>
  <owl:DatatypeProperty rdf:about="http://example.org/onto/prop/google_iam_workforce_pool_delete">
    <rdfs:label>delete</rdfs:label>
    <rdfs:domain rdf:resource="http://example.org/onto/class/google_iam_workforce_pool"/>
    <rdfs:range rdf:resource="http://www.w3.org/2001/XMLSchema#string"/>
  </owl:DatatypeProperty>
  <owl:DatatypeProperty rdf:about="http://example.org/onto/prop/google_iam_workforce_pool_update">
    <rdfs:label>update</rdfs:label>
    <rdfs:domain rdf:resource="http://example.org/onto/class/google_iam_workforce_pool"/>
    <rdfs:range rdf:resource="http://www.w3.org/2001/XMLSchema#string"/>
  </owl:DatatypeProperty>
</rdf:RDF>
