<?xml version="1.0" encoding="UTF-8"?>
<rdf:RDF
  xmlns:rdf="http://www.w3.org/1999/02/22-rdf-syntax-ns#"
  xmlns:rdfs="http://www.w3.org/2000/01/rdf-schema#"
  xmlns:owl="http://www.w3.org/2002/07/owl#"
  xmlns:xsd="http://www.w3.org/2001/XMLSchema#"
  xml:base="http://example.org/onto/">
  <owl:Class rdf:about="http://example.org/onto/class/google_bigquery_capacity_commitment">
    <rdfs:label>google_bigquery_capacity_commitment</rdfs:label>
    <rdfs:comment>#
#     ***     AUTO GENERATED CODE    ***    Type: MMv1     ***
#
# ----------------------------------------------------------------------------
#
#     This code is generated by Magic Modules using the following:
#
#     Configuration: https:#github.com/GoogleCloudPlatform/magic-modules/tree/main/mmv1/products/bigqueryreservation/CapacityCommitment.yaml
#     Template:      https:#github.com/GoogleCloudPlatform/magic-modules/tree/main/mmv1/templates/terraform/resource.html.markdown.tmpl
#
#     DO NOT EDIT this file directly. Any changes made to this file will be
#     overwritten during the next generation cycle.
#
# ----------------------------------------------------------------------------
subcategory: "BigQuery Reservation"
description: |-
  Capacity commitment is a way to purchase compute capacity for BigQuery jobs (in the form of slots) with some committed period of usage.
---</rdfs:comment>
  </owl:Class>
  <owl:DatatypeProperty rdf:about="http://example.org/onto/prop/google_bigquery_capacity_commitment_capacity_commitment_id">
    <rdfs:label>capacity_commitment_id</rdfs:label>
    <rdfs:comment>The optional capacity commitment ID. Capacity commitment name will be generated automatically if this field is
empty. This field must only contain lower case alphanumeric characters or dashes. The first and last character
cannot be a dash. Max length is 64 characters. NOTE: this ID won't be kept if the capacity commitment is split
or merged.</rdfs:comment>
    <rdfs:domain rdf:resource="http://example.org/onto/class/google_bigquery_capacity_commitment"/>
    <rdfs:range rdf:resource="http://www.w3.org/2001/XMLSchema#string"/>
  </owl:DatatypeProperty>
  <owl:DatatypeProperty rdf:about="http://example.org/onto/prop/google_bigquery_capacity_commitment_commitment_end_time">
    <rdfs:label>commitment_end_time</rdfs:label>
    <rdfs:comment>The start of the current commitment period. It is applicable only for ACTIVE capacity commitments.</rdfs:comment>
    <rdfs:domain rdf:resource="http://example.org/onto/class/google_bigquery_capacity_commitment"/>
    <rdfs:range rdf:resource="http://www.w3.org/2001/XMLSchema#string"/>
  </owl:DatatypeProperty>
  <owl:DatatypeProperty rdf:about="http://example.org/onto/prop/google_bigquery_capacity_commitment_commitment_start_time">
    <rdfs:label>commitment_start_time</rdfs:label>
    <rdfs:comment>The start of the current commitment period. It is applicable only for ACTIVE capacity commitments.</rdfs:comment>
    <rdfs:domain rdf:resource="http://example.org/onto/class/google_bigquery_capacity_commitment"/>
    <rdfs:range rdf:resource="http://www.w3.org/2001/XMLSchema#string"/>
  </owl:DatatypeProperty>
  <owl:DatatypeProperty rdf:about="http://example.org/onto/prop/google_bigquery_capacity_commitment_edition">
    <rdfs:label>edition</rdfs:label>
    <rdfs:comment>The edition type. Valid values are STANDARD, ENTERPRISE, ENTERPRISE_PLUS</rdfs:comment>
    <rdfs:domain rdf:resource="http://example.org/onto/class/google_bigquery_capacity_commitment"/>
    <rdfs:range rdf:resource="http://www.w3.org/2001/XMLSchema#string"/>
  </owl:DatatypeProperty>
  <owl:DatatypeProperty rdf:about="http://example.org/onto/prop/google_bigquery_capacity_commitment_enforce_single_admin_project_per_org">
    <rdfs:label>enforce_single_admin_project_per_org</rdfs:label>
    <rdfs:comment>If true, fail the request if another project in the organization has a capacity commitment.</rdfs:comment>
    <rdfs:domain rdf:resource="http://example.org/onto/class/google_bigquery_capacity_commitment"/>
    <rdfs:range rdf:resource="http://www.w3.org/2001/XMLSchema#string"/>
  </owl:DatatypeProperty>
  <owl:DatatypeProperty rdf:about="http://example.org/onto/prop/google_bigquery_capacity_commitment_id">
    <rdfs:label>id</rdfs:label>
    <rdfs:domain rdf:resource="http://example.org/onto/class/google_bigquery_capacity_commitment"/>
    <rdfs:range rdf:resource="http://www.w3.org/2001/XMLSchema#string"/>
  </owl:DatatypeProperty>
  <owl:DatatypeProperty rdf:about="http://example.org/onto/prop/google_bigquery_capacity_commitment_location">
    <rdfs:label>location</rdfs:label>
    <rdfs:comment>The geographic location where the transfer config should reside.
Examples: US, EU, asia-northeast1. The default value is US.</rdfs:comment>
    <rdfs:domain rdf:resource="http://example.org/onto/class/google_bigquery_capacity_commitment"/>
    <rdfs:range rdf:resource="http://www.w3.org/2001/XMLSchema#string"/>
  </owl:DatatypeProperty>
  <owl:DatatypeProperty rdf:about="http://example.org/onto/prop/google_bigquery_capacity_commitment_name">
    <rdfs:label>name</rdfs:label>
    <rdfs:comment>The resource name of the capacity commitment, e.g., projects/myproject/locations/US/capacityCommitments/123</rdfs:comment>
    <rdfs:domain rdf:resource="http://example.org/onto/class/google_bigquery_capacity_commitment"/>
    <rdfs:range rdf:resource="http://www.w3.org/2001/XMLSchema#string"/>
  </owl:DatatypeProperty>
  <owl:DatatypeProperty rdf:about="http://example.org/onto/prop/google_bigquery_capacity_commitment_plan">
    <rdfs:label>plan</rdfs:label>
    <rdfs:comment>Capacity commitment plan. Valid values are at https://cloud.google.com/bigquery/docs/reference/reservations/rpc/google.cloud.bigquery.reservation.v1#commitmentplan</rdfs:comment>
    <rdfs:domain rdf:resource="http://example.org/onto/class/google_bigquery_capacity_commitment"/>
    <rdfs:range rdf:resource="http://www.w3.org/2001/XMLSchema#string"/>
  </owl:DatatypeProperty>
  <owl:DatatypeProperty rdf:about="http://example.org/onto/prop/google_bigquery_capacity_commitment_project">
    <rdfs:label>project</rdfs:label>
    <rdfs:domain rdf:resource="http://example.org/onto/class/google_bigquery_capacity_commitment"/>
    <rdfs:range rdf:resource="http://www.w3.org/2001/XMLSchema#string"/>
  </owl:DatatypeProperty>
  <owl:DatatypeProperty rdf:about="http://example.org/onto/prop/google_bigquery_capacity_commitment_renewal_plan">
    <rdfs:label>renewal_plan</rdfs:label>
    <rdfs:comment>The plan this capacity commitment is converted to after commitmentEndTime passes. Once the plan is changed, committed period is extended according to commitment plan. Only applicable for some commitment plans.</rdfs:comment>
    <rdfs:domain rdf:resource="http://example.org/onto/class/google_bigquery_capacity_commitment"/>
    <rdfs:range rdf:resource="http://www.w3.org/2001/XMLSchema#string"/>
  </owl:DatatypeProperty>
  <owl:DatatypeProperty rdf:about="http://example.org/onto/prop/google_bigquery_capacity_commitment_slot_count">
    <rdfs:label>slot_count</rdfs:label>
    <rdfs:comment>Number of slots in this commitment.</rdfs:comment>
    <rdfs:domain rdf:resource="http://example.org/onto/class/google_bigquery_capacity_commitment"/>
    <rdfs:range rdf:resource="http://www.w3.org/2001/XMLSchema#string"/>
  </owl:DatatypeProperty>
  <owl:DatatypeProperty rdf:about="http://example.org/onto/prop/google_bigquery_capacity_commitment_state">
    <rdfs:label>state</rdfs:label>
    <rdfs:comment>State of the commitment</rdfs:comment>
    <rdfs:domain rdf:resource="http://example.org/onto/class/google_bigquery_capacity_commitment"/>
    <rdfs:range rdf:resource="http://www.w3.org/2001/XMLSchema#string"/>
  </owl:DatatypeProperty>
  <owl:DatatypeProperty rdf:about="http://example.org/onto/prop/google_bigquery_capacity_commitment_create">
    <rdfs:label>create</rdfs:label>
    <rdfs:domain rdf:resource="http://example.org/onto/class/google_bigquery_capacity_commitment"/>
    <rdfs:range rdf:resource="http://www.w3.org/2001/XMLSchema#string"/>
  </owl:DatatypeProperty>
  <owl:DatatypeProperty rdf:about="http://example.org/onto/prop/google_bigquery_capacity_commitment_delete">
    <rdfs:label>delete</rdfs:label>
    <rdfs:domain rdf:resource="http://example.org/onto/class/google_bigquery_capacity_commitment"/>
    <rdfs:range rdf:resource="http://www.w3.org/2001/XMLSchema#string"/>
  </owl:DatatypeProperty>
  <owl:DatatypeProperty rdf:about="http://example.org/onto/prop/google_bigquery_capacity_commitment_update">
    <rdfs:label>update</rdfs:label>
    <rdfs:domain rdf:resource="http://example.org/onto/class/google_bigquery_capacity_commitment"/>
    <rdfs:range rdf:resource="http://www.w3.org/2001/XMLSchema#string"/>
  </owl:DatatypeProperty>
</rdf:RDF>
