<?xml version="1.0" encoding="UTF-8"?>
<rdf:RDF
  xmlns:rdf="http://www.w3.org/1999/02/22-rdf-syntax-ns#"
  xmlns:rdfs="http://www.w3.org/2000/01/rdf-schema#"
  xmlns:owl="http://www.w3.org/2002/07/owl#"
  xmlns:xsd="http://www.w3.org/2001/XMLSchema#"
  xml:base="http://example.org/onto/">
  <owl:Class rdf:about="http://example.org/onto/class/google_model_armor_template">
    <rdfs:label>google_model_armor_template</rdfs:label>
    <rdfs:comment>#
#     ***     AUTO GENERATED CODE    ***    Type: MMv1     ***
#
# ----------------------------------------------------------------------------
#
#     This code is generated by Magic Modules using the following:
#
#     Configuration: https:#github.com/GoogleCloudPlatform/magic-modules/tree/main/mmv1/products/modelarmor/Template.yaml
#     Template:      https:#github.com/GoogleCloudPlatform/magic-modules/tree/main/mmv1/templates/terraform/resource.html.markdown.tmpl
#
#     DO NOT EDIT this file directly. Any changes made to this file will be
#     overwritten during the next generation cycle.
#
# ----------------------------------------------------------------------------
subcategory: "Model Armor"
description: |-
  A `Template` is a resource of Model Armor that lets you configure how Model Armor screens prompts and responses.
---</rdfs:comment>
  </owl:Class>
  <owl:DatatypeProperty rdf:about="http://example.org/onto/prop/google_model_armor_template_create_time">
    <rdfs:label>create_time</rdfs:label>
    <rdfs:comment>Create time stamp</rdfs:comment>
    <rdfs:domain rdf:resource="http://example.org/onto/class/google_model_armor_template"/>
    <rdfs:range rdf:resource="http://www.w3.org/2001/XMLSchema#string"/>
  </owl:DatatypeProperty>
  <owl:DatatypeProperty rdf:about="http://example.org/onto/prop/google_model_armor_template_effective_labels">
    <rdfs:label>effective_labels</rdfs:label>
    <rdfs:comment>All of labels (key/value pairs) present on the resource in GCP, including the labels configured through Terraform, other clients and services.</rdfs:comment>
    <rdfs:domain rdf:resource="http://example.org/onto/class/google_model_armor_template"/>
    <rdfs:range rdf:resource="http://www.w3.org/2001/XMLSchema#string"/>
  </owl:DatatypeProperty>
  <owl:DatatypeProperty rdf:about="http://example.org/onto/prop/google_model_armor_template_id">
    <rdfs:label>id</rdfs:label>
    <rdfs:domain rdf:resource="http://example.org/onto/class/google_model_armor_template"/>
    <rdfs:range rdf:resource="http://www.w3.org/2001/XMLSchema#string"/>
  </owl:DatatypeProperty>
  <owl:DatatypeProperty rdf:about="http://example.org/onto/prop/google_model_armor_template_labels">
    <rdfs:label>labels</rdfs:label>
    <rdfs:comment>Labels as key value pairs

**Note**: This field is non-authoritative, and will only manage the labels present in your configuration.
Please refer to the field 'effective_labels' for all of the labels present on the resource.</rdfs:comment>
    <rdfs:domain rdf:resource="http://example.org/onto/class/google_model_armor_template"/>
    <rdfs:range rdf:resource="http://www.w3.org/2001/XMLSchema#string"/>
  </owl:DatatypeProperty>
  <owl:DatatypeProperty rdf:about="http://example.org/onto/prop/google_model_armor_template_location">
    <rdfs:label>location</rdfs:label>
    <rdfs:comment>Resource ID segment making up resource 'name'. It identifies the resource within its parent collection as described in https://google.aip.dev/122.</rdfs:comment>
    <rdfs:domain rdf:resource="http://example.org/onto/class/google_model_armor_template"/>
    <rdfs:range rdf:resource="http://www.w3.org/2001/XMLSchema#string"/>
  </owl:DatatypeProperty>
  <owl:DatatypeProperty rdf:about="http://example.org/onto/prop/google_model_armor_template_name">
    <rdfs:label>name</rdfs:label>
    <rdfs:comment>Identifier. name of resource</rdfs:comment>
    <rdfs:domain rdf:resource="http://example.org/onto/class/google_model_armor_template"/>
    <rdfs:range rdf:resource="http://www.w3.org/2001/XMLSchema#string"/>
  </owl:DatatypeProperty>
  <owl:DatatypeProperty rdf:about="http://example.org/onto/prop/google_model_armor_template_project">
    <rdfs:label>project</rdfs:label>
    <rdfs:domain rdf:resource="http://example.org/onto/class/google_model_armor_template"/>
    <rdfs:range rdf:resource="http://www.w3.org/2001/XMLSchema#string"/>
  </owl:DatatypeProperty>
  <owl:DatatypeProperty rdf:about="http://example.org/onto/prop/google_model_armor_template_template_id">
    <rdfs:label>template_id</rdfs:label>
    <rdfs:comment>Id of the requesting object
If auto-generating Id server-side, remove this field and
template_id from the method_signature of Create RPC</rdfs:comment>
    <rdfs:domain rdf:resource="http://example.org/onto/class/google_model_armor_template"/>
    <rdfs:range rdf:resource="http://www.w3.org/2001/XMLSchema#string"/>
  </owl:DatatypeProperty>
  <owl:DatatypeProperty rdf:about="http://example.org/onto/prop/google_model_armor_template_terraform_labels">
    <rdfs:label>terraform_labels</rdfs:label>
    <rdfs:comment>The combination of labels configured directly on the resource
 and default labels configured on the provider.</rdfs:comment>
    <rdfs:domain rdf:resource="http://example.org/onto/class/google_model_armor_template"/>
    <rdfs:range rdf:resource="http://www.w3.org/2001/XMLSchema#string"/>
  </owl:DatatypeProperty>
  <owl:DatatypeProperty rdf:about="http://example.org/onto/prop/google_model_armor_template_update_time">
    <rdfs:label>update_time</rdfs:label>
    <rdfs:comment>Update time stamp</rdfs:comment>
    <rdfs:domain rdf:resource="http://example.org/onto/class/google_model_armor_template"/>
    <rdfs:range rdf:resource="http://www.w3.org/2001/XMLSchema#string"/>
  </owl:DatatypeProperty>
  <owl:DatatypeProperty rdf:about="http://example.org/onto/prop/google_model_armor_template_filter_enforcement">
    <rdfs:label>filter_enforcement</rdfs:label>
    <rdfs:comment>Tells whether the Malicious URI filter is enabled or disabled.
Possible values:
ENABLED
DISABLED</rdfs:comment>
    <rdfs:domain rdf:resource="http://example.org/onto/class/google_model_armor_template"/>
    <rdfs:range rdf:resource="http://www.w3.org/2001/XMLSchema#string"/>
  </owl:DatatypeProperty>
  <owl:DatatypeProperty rdf:about="http://example.org/onto/prop/google_model_armor_template_confidence_level">
    <rdfs:label>confidence_level</rdfs:label>
    <rdfs:comment>Possible values:
LOW_AND_ABOVE
MEDIUM_AND_ABOVE
HIGH</rdfs:comment>
    <rdfs:domain rdf:resource="http://example.org/onto/class/google_model_armor_template"/>
    <rdfs:range rdf:resource="http://www.w3.org/2001/XMLSchema#string"/>
  </owl:DatatypeProperty>
  <owl:DatatypeProperty rdf:about="http://example.org/onto/prop/google_model_armor_template_filter_enforcement">
    <rdfs:label>filter_enforcement</rdfs:label>
    <rdfs:comment>Tells whether Prompt injection and Jailbreak filter is enabled or
disabled.
Possible values:
ENABLED
DISABLED</rdfs:comment>
    <rdfs:domain rdf:resource="http://example.org/onto/class/google_model_armor_template"/>
    <rdfs:range rdf:resource="http://www.w3.org/2001/XMLSchema#string"/>
  </owl:DatatypeProperty>
  <owl:DatatypeProperty rdf:about="http://example.org/onto/prop/google_model_armor_template_confidence_level">
    <rdfs:label>confidence_level</rdfs:label>
    <rdfs:comment>Possible values:
LOW_AND_ABOVE
MEDIUM_AND_ABOVE
HIGH</rdfs:comment>
    <rdfs:domain rdf:resource="http://example.org/onto/class/google_model_armor_template"/>
    <rdfs:range rdf:resource="http://www.w3.org/2001/XMLSchema#string"/>
  </owl:DatatypeProperty>
  <owl:DatatypeProperty rdf:about="http://example.org/onto/prop/google_model_armor_template_filter_type">
    <rdfs:label>filter_type</rdfs:label>
    <rdfs:comment>Possible values:
SEXUALLY_EXPLICIT
HATE_SPEECH
HARASSMENT
DANGEROUS</rdfs:comment>
    <rdfs:domain rdf:resource="http://example.org/onto/class/google_model_armor_template"/>
    <rdfs:range rdf:resource="http://www.w3.org/2001/XMLSchema#string"/>
  </owl:DatatypeProperty>
  <owl:DatatypeProperty rdf:about="http://example.org/onto/prop/google_model_armor_template_deidentify_template">
    <rdfs:label>deidentify_template</rdfs:label>
    <rdfs:comment>Optional Sensitive Data Protection Deidentify template resource name.
If provided then DeidentifyContent action is performed during Sanitization
using this template and inspect template. The De-identified data will
be returned in SdpDeidentifyResult.
Note that all info-types present in the deidentify template must be present
in inspect template.
e.g.
'projects/{project}/locations/{location}/deidentifyTemplates/{deidentify_template}'</rdfs:comment>
    <rdfs:domain rdf:resource="http://example.org/onto/class/google_model_armor_template"/>
    <rdfs:range rdf:resource="http://www.w3.org/2001/XMLSchema#string"/>
  </owl:DatatypeProperty>
  <owl:DatatypeProperty rdf:about="http://example.org/onto/prop/google_model_armor_template_inspect_template">
    <rdfs:label>inspect_template</rdfs:label>
    <rdfs:comment>Sensitive Data Protection inspect template resource name
If only inspect template is provided (de-identify template not provided),
then Sensitive Data Protection InspectContent action is performed during
Sanitization. All Sensitive Data Protection findings identified during
inspection will be returned as SdpFinding in SdpInsepctionResult.
e.g:-
'projects/{project}/locations/{location}/inspectTemplates/{inspect_template}'</rdfs:comment>
    <rdfs:domain rdf:resource="http://example.org/onto/class/google_model_armor_template"/>
    <rdfs:range rdf:resource="http://www.w3.org/2001/XMLSchema#string"/>
  </owl:DatatypeProperty>
  <owl:DatatypeProperty rdf:about="http://example.org/onto/prop/google_model_armor_template_filter_enforcement">
    <rdfs:label>filter_enforcement</rdfs:label>
    <rdfs:comment>Tells whether the Sensitive Data Protection basic config is enabled or
disabled.
Possible values:
ENABLED
DISABLED</rdfs:comment>
    <rdfs:domain rdf:resource="http://example.org/onto/class/google_model_armor_template"/>
    <rdfs:range rdf:resource="http://www.w3.org/2001/XMLSchema#string"/>
  </owl:DatatypeProperty>
  <owl:DatatypeProperty rdf:about="http://example.org/onto/prop/google_model_armor_template_custom_llm_response_safety_error_code">
    <rdfs:label>custom_llm_response_safety_error_code</rdfs:label>
    <rdfs:comment>Indicates the custom error code set by the user to be returned to the end
user if the LLM response trips Model Armor filters.</rdfs:comment>
    <rdfs:domain rdf:resource="http://example.org/onto/class/google_model_armor_template"/>
    <rdfs:range rdf:resource="http://www.w3.org/2001/XMLSchema#string"/>
  </owl:DatatypeProperty>
  <owl:DatatypeProperty rdf:about="http://example.org/onto/prop/google_model_armor_template_custom_llm_response_safety_error_message">
    <rdfs:label>custom_llm_response_safety_error_message</rdfs:label>
    <rdfs:comment>Indicates the custom error message set by the user to be returned to the
end user if the LLM response trips Model Armor filters.</rdfs:comment>
    <rdfs:domain rdf:resource="http://example.org/onto/class/google_model_armor_template"/>
    <rdfs:range rdf:resource="http://www.w3.org/2001/XMLSchema#string"/>
  </owl:DatatypeProperty>
  <owl:DatatypeProperty rdf:about="http://example.org/onto/prop/google_model_armor_template_custom_prompt_safety_error_code">
    <rdfs:label>custom_prompt_safety_error_code</rdfs:label>
    <rdfs:comment>Indicates the custom error code set by the user to be returned to the end
user by the service extension if the prompt trips Model Armor filters.</rdfs:comment>
    <rdfs:domain rdf:resource="http://example.org/onto/class/google_model_armor_template"/>
    <rdfs:range rdf:resource="http://www.w3.org/2001/XMLSchema#string"/>
  </owl:DatatypeProperty>
  <owl:DatatypeProperty rdf:about="http://example.org/onto/prop/google_model_armor_template_custom_prompt_safety_error_message">
    <rdfs:label>custom_prompt_safety_error_message</rdfs:label>
    <rdfs:comment>Indicates the custom error message set by the user to be returned to the
end user if the prompt trips Model Armor filters.</rdfs:comment>
    <rdfs:domain rdf:resource="http://example.org/onto/class/google_model_armor_template"/>
    <rdfs:range rdf:resource="http://www.w3.org/2001/XMLSchema#string"/>
  </owl:DatatypeProperty>
  <owl:DatatypeProperty rdf:about="http://example.org/onto/prop/google_model_armor_template_enforcement_type">
    <rdfs:label>enforcement_type</rdfs:label>
    <rdfs:comment>Possible values:
INSPECT_ONLY
INSPECT_AND_BLOCK</rdfs:comment>
    <rdfs:domain rdf:resource="http://example.org/onto/class/google_model_armor_template"/>
    <rdfs:range rdf:resource="http://www.w3.org/2001/XMLSchema#string"/>
  </owl:DatatypeProperty>
  <owl:DatatypeProperty rdf:about="http://example.org/onto/prop/google_model_armor_template_ignore_partial_invocation_failures">
    <rdfs:label>ignore_partial_invocation_failures</rdfs:label>
    <rdfs:comment>If true, partial detector failures should be ignored.</rdfs:comment>
    <rdfs:domain rdf:resource="http://example.org/onto/class/google_model_armor_template"/>
    <rdfs:range rdf:resource="http://www.w3.org/2001/XMLSchema#string"/>
  </owl:DatatypeProperty>
  <owl:DatatypeProperty rdf:about="http://example.org/onto/prop/google_model_armor_template_log_sanitize_operations">
    <rdfs:label>log_sanitize_operations</rdfs:label>
    <rdfs:comment>If true, log sanitize operations.</rdfs:comment>
    <rdfs:domain rdf:resource="http://example.org/onto/class/google_model_armor_template"/>
    <rdfs:range rdf:resource="http://www.w3.org/2001/XMLSchema#string"/>
  </owl:DatatypeProperty>
  <owl:DatatypeProperty rdf:about="http://example.org/onto/prop/google_model_armor_template_log_template_operations">
    <rdfs:label>log_template_operations</rdfs:label>
    <rdfs:comment>If true, log template crud operations.</rdfs:comment>
    <rdfs:domain rdf:resource="http://example.org/onto/class/google_model_armor_template"/>
    <rdfs:range rdf:resource="http://www.w3.org/2001/XMLSchema#string"/>
  </owl:DatatypeProperty>
  <owl:DatatypeProperty rdf:about="http://example.org/onto/prop/google_model_armor_template_enable_multi_language_detection">
    <rdfs:label>enable_multi_language_detection</rdfs:label>
    <rdfs:comment>If true, multi language detection will be enabled.</rdfs:comment>
    <rdfs:domain rdf:resource="http://example.org/onto/class/google_model_armor_template"/>
    <rdfs:range rdf:resource="http://www.w3.org/2001/XMLSchema#string"/>
  </owl:DatatypeProperty>
  <owl:DatatypeProperty rdf:about="http://example.org/onto/prop/google_model_armor_template_create">
    <rdfs:label>create</rdfs:label>
    <rdfs:domain rdf:resource="http://example.org/onto/class/google_model_armor_template"/>
    <rdfs:range rdf:resource="http://www.w3.org/2001/XMLSchema#string"/>
  </owl:DatatypeProperty>
  <owl:DatatypeProperty rdf:about="http://example.org/onto/prop/google_model_armor_template_delete">
    <rdfs:label>delete</rdfs:label>
    <rdfs:domain rdf:resource="http://example.org/onto/class/google_model_armor_template"/>
    <rdfs:range rdf:resource="http://www.w3.org/2001/XMLSchema#string"/>
  </owl:DatatypeProperty>
  <owl:DatatypeProperty rdf:about="http://example.org/onto/prop/google_model_armor_template_update">
    <rdfs:label>update</rdfs:label>
    <rdfs:domain rdf:resource="http://example.org/onto/class/google_model_armor_template"/>
    <rdfs:range rdf:resource="http://www.w3.org/2001/XMLSchema#string"/>
  </owl:DatatypeProperty>
</rdf:RDF>
