<?xml version="1.0" encoding="UTF-8"?>
<rdf:RDF
  xmlns:rdf="http://www.w3.org/1999/02/22-rdf-syntax-ns#"
  xmlns:rdfs="http://www.w3.org/2000/01/rdf-schema#"
  xmlns:owl="http://www.w3.org/2002/07/owl#"
  xmlns:xsd="http://www.w3.org/2001/XMLSchema#"
  xml:base="http://example.org/onto/">
  <owl:Class rdf:about="http://example.org/onto/class/google_container_node_pool">
    <rdfs:label>google_container_node_pool</rdfs:label>
    <rdfs:comment>#
#     ***     AUTO GENERATED CODE    ***    Type: Handwritten     ***
#
# ----------------------------------------------------------------------------
#
#     This code is generated by Magic Modules using the following:
#
#     Source file: https://github.com/GoogleCloudPlatform/magic-modules/tree/main/mmv1/third_party/terraform/website/docs/r/container_node_pool.html.markdown
#
#     DO NOT EDIT this file directly. Any changes made to this file will be
#     overwritten during the next generation cycle.
#
# ----------------------------------------------------------------------------
subcategory: "Kubernetes (Container) Engine"
description: |-
  Manages a GKE NodePool resource.
---</rdfs:comment>
  </owl:Class>
  <owl:DatatypeProperty rdf:about="http://example.org/onto/prop/google_container_node_pool_cluster">
    <rdfs:label>cluster</rdfs:label>
    <rdfs:comment>The cluster to create the node pool for. Cluster must be present in location provided for zonal clusters.</rdfs:comment>
    <rdfs:domain rdf:resource="http://example.org/onto/class/google_container_node_pool"/>
    <rdfs:range rdf:resource="http://www.w3.org/2001/XMLSchema#string"/>
  </owl:DatatypeProperty>
  <owl:DatatypeProperty rdf:about="http://example.org/onto/prop/google_container_node_pool_id">
    <rdfs:label>id</rdfs:label>
    <rdfs:domain rdf:resource="http://example.org/onto/class/google_container_node_pool"/>
    <rdfs:range rdf:resource="http://www.w3.org/2001/XMLSchema#string"/>
  </owl:DatatypeProperty>
  <owl:DatatypeProperty rdf:about="http://example.org/onto/prop/google_container_node_pool_initial_node_count">
    <rdfs:label>initial_node_count</rdfs:label>
    <rdfs:comment>The initial number of nodes for the pool. In regional or multi-zonal clusters, this is the number of nodes per zone. Changing this will force recreation of the resource.</rdfs:comment>
    <rdfs:domain rdf:resource="http://example.org/onto/class/google_container_node_pool"/>
    <rdfs:range rdf:resource="http://www.w3.org/2001/XMLSchema#string"/>
  </owl:DatatypeProperty>
  <owl:DatatypeProperty rdf:about="http://example.org/onto/prop/google_container_node_pool_instance_group_urls">
    <rdfs:label>instance_group_urls</rdfs:label>
    <rdfs:comment>The resource URLs of the managed instance groups associated with this node pool.</rdfs:comment>
    <rdfs:domain rdf:resource="http://example.org/onto/class/google_container_node_pool"/>
    <rdfs:range rdf:resource="http://www.w3.org/2001/XMLSchema#string"/>
  </owl:DatatypeProperty>
  <owl:DatatypeProperty rdf:about="http://example.org/onto/prop/google_container_node_pool_location">
    <rdfs:label>location</rdfs:label>
    <rdfs:comment>The location (region or zone) of the cluster.</rdfs:comment>
    <rdfs:domain rdf:resource="http://example.org/onto/class/google_container_node_pool"/>
    <rdfs:range rdf:resource="http://www.w3.org/2001/XMLSchema#string"/>
  </owl:DatatypeProperty>
  <owl:DatatypeProperty rdf:about="http://example.org/onto/prop/google_container_node_pool_managed_instance_group_urls">
    <rdfs:label>managed_instance_group_urls</rdfs:label>
    <rdfs:comment>List of instance group URLs which have been assigned to this node pool.</rdfs:comment>
    <rdfs:domain rdf:resource="http://example.org/onto/class/google_container_node_pool"/>
    <rdfs:range rdf:resource="http://www.w3.org/2001/XMLSchema#string"/>
  </owl:DatatypeProperty>
  <owl:DatatypeProperty rdf:about="http://example.org/onto/prop/google_container_node_pool_max_pods_per_node">
    <rdfs:label>max_pods_per_node</rdfs:label>
    <rdfs:comment>The maximum number of pods per node in this node pool. Note that this does not work on node pools which are "route-based" - that is, node pools belonging to clusters that do not have IP Aliasing enabled.</rdfs:comment>
    <rdfs:domain rdf:resource="http://example.org/onto/class/google_container_node_pool"/>
    <rdfs:range rdf:resource="http://www.w3.org/2001/XMLSchema#string"/>
  </owl:DatatypeProperty>
  <owl:DatatypeProperty rdf:about="http://example.org/onto/prop/google_container_node_pool_name">
    <rdfs:label>name</rdfs:label>
    <rdfs:comment>The name of the node pool. If left blank, Terraform will auto-generate a unique name.</rdfs:comment>
    <rdfs:domain rdf:resource="http://example.org/onto/class/google_container_node_pool"/>
    <rdfs:range rdf:resource="http://www.w3.org/2001/XMLSchema#string"/>
  </owl:DatatypeProperty>
  <owl:DatatypeProperty rdf:about="http://example.org/onto/prop/google_container_node_pool_name_prefix">
    <rdfs:label>name_prefix</rdfs:label>
    <rdfs:comment>Creates a unique name for the node pool beginning with the specified prefix. Conflicts with name.</rdfs:comment>
    <rdfs:domain rdf:resource="http://example.org/onto/class/google_container_node_pool"/>
    <rdfs:range rdf:resource="http://www.w3.org/2001/XMLSchema#string"/>
  </owl:DatatypeProperty>
  <owl:DatatypeProperty rdf:about="http://example.org/onto/prop/google_container_node_pool_node_count">
    <rdfs:label>node_count</rdfs:label>
    <rdfs:comment>The number of nodes per instance group. This field can be used to update the number of nodes per instance group but should not be used alongside autoscaling.</rdfs:comment>
    <rdfs:domain rdf:resource="http://example.org/onto/class/google_container_node_pool"/>
    <rdfs:range rdf:resource="http://www.w3.org/2001/XMLSchema#string"/>
  </owl:DatatypeProperty>
  <owl:DatatypeProperty rdf:about="http://example.org/onto/prop/google_container_node_pool_node_locations">
    <rdfs:label>node_locations</rdfs:label>
    <rdfs:comment>The list of zones in which the node pool's nodes should be located. Nodes must be in the region of their regional cluster or in the same region as their cluster's zone for zonal clusters. If unspecified, the cluster-level node_locations will be used.</rdfs:comment>
    <rdfs:domain rdf:resource="http://example.org/onto/class/google_container_node_pool"/>
    <rdfs:range rdf:resource="http://www.w3.org/2001/XMLSchema#string"/>
  </owl:DatatypeProperty>
  <owl:DatatypeProperty rdf:about="http://example.org/onto/prop/google_container_node_pool_operation">
    <rdfs:label>operation</rdfs:label>
    <rdfs:domain rdf:resource="http://example.org/onto/class/google_container_node_pool"/>
    <rdfs:range rdf:resource="http://www.w3.org/2001/XMLSchema#string"/>
  </owl:DatatypeProperty>
  <owl:DatatypeProperty rdf:about="http://example.org/onto/prop/google_container_node_pool_project">
    <rdfs:label>project</rdfs:label>
    <rdfs:comment>The ID of the project in which to create the node pool. If blank, the provider-configured project will be used.</rdfs:comment>
    <rdfs:domain rdf:resource="http://example.org/onto/class/google_container_node_pool"/>
    <rdfs:range rdf:resource="http://www.w3.org/2001/XMLSchema#string"/>
  </owl:DatatypeProperty>
  <owl:DatatypeProperty rdf:about="http://example.org/onto/prop/google_container_node_pool_version">
    <rdfs:label>version</rdfs:label>
    <rdfs:comment>The Kubernetes version for the nodes in this pool. Note that if this field and auto_upgrade are both specified, they will fight each other for what the node version should be, so setting both is highly discouraged. While a fuzzy version can be specified, it's recommended that you specify explicit versions as Terraform will see spurious diffs when fuzzy versions are used. See the google_container_engine_versions data source's version_prefix field to approximate fuzzy versions in a Terraform-compatible way.</rdfs:comment>
    <rdfs:domain rdf:resource="http://example.org/onto/class/google_container_node_pool"/>
    <rdfs:range rdf:resource="http://www.w3.org/2001/XMLSchema#string"/>
  </owl:DatatypeProperty>
  <owl:DatatypeProperty rdf:about="http://example.org/onto/prop/google_container_node_pool_location_policy">
    <rdfs:label>location_policy</rdfs:label>
    <rdfs:comment>Location policy specifies the algorithm used when scaling-up the node pool. "BALANCED" - Is a best effort policy that aims to balance the sizes of available zones. "ANY" - Instructs the cluster autoscaler to prioritize utilization of unused reservations, and reduces preemption risk for Spot VMs.</rdfs:comment>
    <rdfs:domain rdf:resource="http://example.org/onto/class/google_container_node_pool"/>
    <rdfs:range rdf:resource="http://www.w3.org/2001/XMLSchema#string"/>
  </owl:DatatypeProperty>
  <owl:DatatypeProperty rdf:about="http://example.org/onto/prop/google_container_node_pool_max_node_count">
    <rdfs:label>max_node_count</rdfs:label>
    <rdfs:comment>Maximum number of nodes per zone in the node pool. Must be >= min_node_count. Cannot be used with total limits.</rdfs:comment>
    <rdfs:domain rdf:resource="http://example.org/onto/class/google_container_node_pool"/>
    <rdfs:range rdf:resource="http://www.w3.org/2001/XMLSchema#string"/>
  </owl:DatatypeProperty>
  <owl:DatatypeProperty rdf:about="http://example.org/onto/prop/google_container_node_pool_min_node_count">
    <rdfs:label>min_node_count</rdfs:label>
    <rdfs:comment>Minimum number of nodes per zone in the node pool. Must be >=0 and <= max_node_count. Cannot be used with total limits.</rdfs:comment>
    <rdfs:domain rdf:resource="http://example.org/onto/class/google_container_node_pool"/>
    <rdfs:range rdf:resource="http://www.w3.org/2001/XMLSchema#string"/>
  </owl:DatatypeProperty>
  <owl:DatatypeProperty rdf:about="http://example.org/onto/prop/google_container_node_pool_total_max_node_count">
    <rdfs:label>total_max_node_count</rdfs:label>
    <rdfs:comment>Maximum number of all nodes in the node pool. Must be >= total_min_node_count. Cannot be used with per zone limits.</rdfs:comment>
    <rdfs:domain rdf:resource="http://example.org/onto/class/google_container_node_pool"/>
    <rdfs:range rdf:resource="http://www.w3.org/2001/XMLSchema#string"/>
  </owl:DatatypeProperty>
  <owl:DatatypeProperty rdf:about="http://example.org/onto/prop/google_container_node_pool_total_min_node_count">
    <rdfs:label>total_min_node_count</rdfs:label>
    <rdfs:comment>Minimum number of all nodes in the node pool. Must be >=0 and <= total_max_node_count. Cannot be used with per zone limits.</rdfs:comment>
    <rdfs:domain rdf:resource="http://example.org/onto/class/google_container_node_pool"/>
    <rdfs:range rdf:resource="http://www.w3.org/2001/XMLSchema#string"/>
  </owl:DatatypeProperty>
  <owl:DatatypeProperty rdf:about="http://example.org/onto/prop/google_container_node_pool_auto_repair">
    <rdfs:label>auto_repair</rdfs:label>
    <rdfs:comment>Whether the nodes will be automatically repaired. Enabled by default.</rdfs:comment>
    <rdfs:domain rdf:resource="http://example.org/onto/class/google_container_node_pool"/>
    <rdfs:range rdf:resource="http://www.w3.org/2001/XMLSchema#string"/>
  </owl:DatatypeProperty>
  <owl:DatatypeProperty rdf:about="http://example.org/onto/prop/google_container_node_pool_auto_upgrade">
    <rdfs:label>auto_upgrade</rdfs:label>
    <rdfs:comment>Whether the nodes will be automatically upgraded. Enabled by default.</rdfs:comment>
    <rdfs:domain rdf:resource="http://example.org/onto/class/google_container_node_pool"/>
    <rdfs:range rdf:resource="http://www.w3.org/2001/XMLSchema#string"/>
  </owl:DatatypeProperty>
  <owl:DatatypeProperty rdf:about="http://example.org/onto/prop/google_container_node_pool_create_pod_range">
    <rdfs:label>create_pod_range</rdfs:label>
    <rdfs:comment>Whether to create a new range for pod IPs in this node pool. Defaults are provided for pod_range and pod_ipv4_cidr_block if they are not specified.</rdfs:comment>
    <rdfs:domain rdf:resource="http://example.org/onto/class/google_container_node_pool"/>
    <rdfs:range rdf:resource="http://www.w3.org/2001/XMLSchema#string"/>
  </owl:DatatypeProperty>
  <owl:DatatypeProperty rdf:about="http://example.org/onto/prop/google_container_node_pool_enable_private_nodes">
    <rdfs:label>enable_private_nodes</rdfs:label>
    <rdfs:comment>Whether nodes have internal IP addresses only.</rdfs:comment>
    <rdfs:domain rdf:resource="http://example.org/onto/class/google_container_node_pool"/>
    <rdfs:range rdf:resource="http://www.w3.org/2001/XMLSchema#string"/>
  </owl:DatatypeProperty>
  <owl:DatatypeProperty rdf:about="http://example.org/onto/prop/google_container_node_pool_pod_ipv4_cidr_block">
    <rdfs:label>pod_ipv4_cidr_block</rdfs:label>
    <rdfs:comment>The IP address range for pod IPs in this node pool. Only applicable if create_pod_range is true. Set to blank to have a range chosen with the default size. Set to /netmask (e.g. /14) to have a range chosen with a specific netmask. Set to a CIDR notation (e.g. 10.96.0.0/14) to pick a specific range to use.</rdfs:comment>
    <rdfs:domain rdf:resource="http://example.org/onto/class/google_container_node_pool"/>
    <rdfs:range rdf:resource="http://www.w3.org/2001/XMLSchema#string"/>
  </owl:DatatypeProperty>
  <owl:DatatypeProperty rdf:about="http://example.org/onto/prop/google_container_node_pool_pod_range">
    <rdfs:label>pod_range</rdfs:label>
    <rdfs:comment>The ID of the secondary range for pod IPs. If create_pod_range is true, this ID is used for the new range. If create_pod_range is false, uses an existing secondary range with this ID.</rdfs:comment>
    <rdfs:domain rdf:resource="http://example.org/onto/class/google_container_node_pool"/>
    <rdfs:range rdf:resource="http://www.w3.org/2001/XMLSchema#string"/>
  </owl:DatatypeProperty>
  <owl:DatatypeProperty rdf:about="http://example.org/onto/prop/google_container_node_pool_subnetwork">
    <rdfs:label>subnetwork</rdfs:label>
    <rdfs:comment>The subnetwork path for the node pool. Format: projects/{project}/regions/{region}/subnetworks/{subnetwork} . If the cluster is associated with multiple subnetworks, the subnetwork for the node pool is picked based on the IP utilization during node pool creation and is immutable.</rdfs:comment>
    <rdfs:domain rdf:resource="http://example.org/onto/class/google_container_node_pool"/>
    <rdfs:range rdf:resource="http://www.w3.org/2001/XMLSchema#string"/>
  </owl:DatatypeProperty>
  <owl:DatatypeProperty rdf:about="http://example.org/onto/prop/google_container_node_pool_network">
    <rdfs:label>network</rdfs:label>
    <rdfs:comment>Name of the VPC where the additional interface belongs.</rdfs:comment>
    <rdfs:domain rdf:resource="http://example.org/onto/class/google_container_node_pool"/>
    <rdfs:range rdf:resource="http://www.w3.org/2001/XMLSchema#string"/>
  </owl:DatatypeProperty>
  <owl:DatatypeProperty rdf:about="http://example.org/onto/prop/google_container_node_pool_subnetwork">
    <rdfs:label>subnetwork</rdfs:label>
    <rdfs:comment>Name of the subnetwork where the additional interface belongs.</rdfs:comment>
    <rdfs:domain rdf:resource="http://example.org/onto/class/google_container_node_pool"/>
    <rdfs:range rdf:resource="http://www.w3.org/2001/XMLSchema#string"/>
  </owl:DatatypeProperty>
  <owl:DatatypeProperty rdf:about="http://example.org/onto/prop/google_container_node_pool_max_pods_per_node">
    <rdfs:label>max_pods_per_node</rdfs:label>
    <rdfs:comment>The maximum number of pods per node which use this pod network.</rdfs:comment>
    <rdfs:domain rdf:resource="http://example.org/onto/class/google_container_node_pool"/>
    <rdfs:range rdf:resource="http://www.w3.org/2001/XMLSchema#string"/>
  </owl:DatatypeProperty>
  <owl:DatatypeProperty rdf:about="http://example.org/onto/prop/google_container_node_pool_secondary_pod_range">
    <rdfs:label>secondary_pod_range</rdfs:label>
    <rdfs:comment>The name of the secondary range on the subnet which provides IP address for this pod range.</rdfs:comment>
    <rdfs:domain rdf:resource="http://example.org/onto/class/google_container_node_pool"/>
    <rdfs:range rdf:resource="http://www.w3.org/2001/XMLSchema#string"/>
  </owl:DatatypeProperty>
  <owl:DatatypeProperty rdf:about="http://example.org/onto/prop/google_container_node_pool_subnetwork">
    <rdfs:label>subnetwork</rdfs:label>
    <rdfs:comment>Name of the subnetwork where the additional pod network belongs.</rdfs:comment>
    <rdfs:domain rdf:resource="http://example.org/onto/class/google_container_node_pool"/>
    <rdfs:range rdf:resource="http://www.w3.org/2001/XMLSchema#string"/>
  </owl:DatatypeProperty>
  <owl:DatatypeProperty rdf:about="http://example.org/onto/prop/google_container_node_pool_total_egress_bandwidth_tier">
    <rdfs:label>total_egress_bandwidth_tier</rdfs:label>
    <rdfs:comment>Specifies the total network bandwidth tier for the NodePool. [Valid values](https://cloud.google.com/kubernetes-engine/docs/reference/rest/v1/projects.locations.clusters.nodePools#NodePool.Tier) include: "TIER_1" and "TIER_UNSPECIFIED".</rdfs:comment>
    <rdfs:domain rdf:resource="http://example.org/onto/class/google_container_node_pool"/>
    <rdfs:range rdf:resource="http://www.w3.org/2001/XMLSchema#string"/>
  </owl:DatatypeProperty>
  <owl:DatatypeProperty rdf:about="http://example.org/onto/prop/google_container_node_pool_disabled">
    <rdfs:label>disabled</rdfs:label>
    <rdfs:domain rdf:resource="http://example.org/onto/class/google_container_node_pool"/>
    <rdfs:range rdf:resource="http://www.w3.org/2001/XMLSchema#string"/>
  </owl:DatatypeProperty>
  <owl:DatatypeProperty rdf:about="http://example.org/onto/prop/google_container_node_pool_boot_disk_kms_key">
    <rdfs:label>boot_disk_kms_key</rdfs:label>
    <rdfs:comment>The Customer Managed Encryption Key used to encrypt the boot disk attached to each node in the node pool.</rdfs:comment>
    <rdfs:domain rdf:resource="http://example.org/onto/class/google_container_node_pool"/>
    <rdfs:range rdf:resource="http://www.w3.org/2001/XMLSchema#string"/>
  </owl:DatatypeProperty>
  <owl:DatatypeProperty rdf:about="http://example.org/onto/prop/google_container_node_pool_disk_size_gb">
    <rdfs:label>disk_size_gb</rdfs:label>
    <rdfs:comment>Size of the disk attached to each node, specified in GB. The smallest allowed disk size is 10GB.</rdfs:comment>
    <rdfs:domain rdf:resource="http://example.org/onto/class/google_container_node_pool"/>
    <rdfs:range rdf:resource="http://www.w3.org/2001/XMLSchema#string"/>
  </owl:DatatypeProperty>
  <owl:DatatypeProperty rdf:about="http://example.org/onto/prop/google_container_node_pool_disk_type">
    <rdfs:label>disk_type</rdfs:label>
    <rdfs:comment>Type of the disk attached to each node. Such as pd-standard, pd-balanced or pd-ssd</rdfs:comment>
    <rdfs:domain rdf:resource="http://example.org/onto/class/google_container_node_pool"/>
    <rdfs:range rdf:resource="http://www.w3.org/2001/XMLSchema#string"/>
  </owl:DatatypeProperty>
  <owl:DatatypeProperty rdf:about="http://example.org/onto/prop/google_container_node_pool_effective_taints">
    <rdfs:label>effective_taints</rdfs:label>
    <rdfs:comment>List of kubernetes taints applied to each node.</rdfs:comment>
    <rdfs:domain rdf:resource="http://example.org/onto/class/google_container_node_pool"/>
    <rdfs:range rdf:resource="http://www.w3.org/2001/XMLSchema#string"/>
  </owl:DatatypeProperty>
  <owl:DatatypeProperty rdf:about="http://example.org/onto/prop/google_container_node_pool_enable_confidential_storage">
    <rdfs:label>enable_confidential_storage</rdfs:label>
    <rdfs:comment>If enabled boot disks are configured with confidential mode.</rdfs:comment>
    <rdfs:domain rdf:resource="http://example.org/onto/class/google_container_node_pool"/>
    <rdfs:range rdf:resource="http://www.w3.org/2001/XMLSchema#string"/>
  </owl:DatatypeProperty>
  <owl:DatatypeProperty rdf:about="http://example.org/onto/prop/google_container_node_pool_flex_start">
    <rdfs:label>flex_start</rdfs:label>
    <rdfs:comment>Enables Flex Start provisioning model for the node pool</rdfs:comment>
    <rdfs:domain rdf:resource="http://example.org/onto/class/google_container_node_pool"/>
    <rdfs:range rdf:resource="http://www.w3.org/2001/XMLSchema#string"/>
  </owl:DatatypeProperty>
  <owl:DatatypeProperty rdf:about="http://example.org/onto/prop/google_container_node_pool_image_type">
    <rdfs:label>image_type</rdfs:label>
    <rdfs:comment>The image type to use for this node. Note that for a given image type, the latest version of it will be used.</rdfs:comment>
    <rdfs:domain rdf:resource="http://example.org/onto/class/google_container_node_pool"/>
    <rdfs:range rdf:resource="http://www.w3.org/2001/XMLSchema#string"/>
  </owl:DatatypeProperty>
  <owl:DatatypeProperty rdf:about="http://example.org/onto/prop/google_container_node_pool_labels">
    <rdfs:label>labels</rdfs:label>
    <rdfs:comment>The map of Kubernetes labels (key/value pairs) to be applied to each node. These will added in addition to any default label(s) that Kubernetes may apply to the node.</rdfs:comment>
    <rdfs:domain rdf:resource="http://example.org/onto/class/google_container_node_pool"/>
    <rdfs:range rdf:resource="http://www.w3.org/2001/XMLSchema#string"/>
  </owl:DatatypeProperty>
  <owl:DatatypeProperty rdf:about="http://example.org/onto/prop/google_container_node_pool_local_ssd_count">
    <rdfs:label>local_ssd_count</rdfs:label>
    <rdfs:comment>The number of local SSD disks to be attached to the node.</rdfs:comment>
    <rdfs:domain rdf:resource="http://example.org/onto/class/google_container_node_pool"/>
    <rdfs:range rdf:resource="http://www.w3.org/2001/XMLSchema#string"/>
  </owl:DatatypeProperty>
  <owl:DatatypeProperty rdf:about="http://example.org/onto/prop/google_container_node_pool_local_ssd_encryption_mode">
    <rdfs:label>local_ssd_encryption_mode</rdfs:label>
    <rdfs:comment>LocalSsdEncryptionMode specified the method used for encrypting the local SSDs attached to the node.</rdfs:comment>
    <rdfs:domain rdf:resource="http://example.org/onto/class/google_container_node_pool"/>
    <rdfs:range rdf:resource="http://www.w3.org/2001/XMLSchema#string"/>
  </owl:DatatypeProperty>
  <owl:DatatypeProperty rdf:about="http://example.org/onto/prop/google_container_node_pool_logging_variant">
    <rdfs:label>logging_variant</rdfs:label>
    <rdfs:comment>Type of logging agent that is used as the default value for node pools in the cluster. Valid values include DEFAULT and MAX_THROUGHPUT.</rdfs:comment>
    <rdfs:domain rdf:resource="http://example.org/onto/class/google_container_node_pool"/>
    <rdfs:range rdf:resource="http://www.w3.org/2001/XMLSchema#string"/>
  </owl:DatatypeProperty>
  <owl:DatatypeProperty rdf:about="http://example.org/onto/prop/google_container_node_pool_machine_type">
    <rdfs:label>machine_type</rdfs:label>
    <rdfs:comment>The name of a Google Compute Engine machine type.</rdfs:comment>
    <rdfs:domain rdf:resource="http://example.org/onto/class/google_container_node_pool"/>
    <rdfs:range rdf:resource="http://www.w3.org/2001/XMLSchema#string"/>
  </owl:DatatypeProperty>
  <owl:DatatypeProperty rdf:about="http://example.org/onto/prop/google_container_node_pool_max_run_duration">
    <rdfs:label>max_run_duration</rdfs:label>
    <rdfs:comment>The runtime of each node in the node pool in seconds, terminated by 's'. Example: "3600s".</rdfs:comment>
    <rdfs:domain rdf:resource="http://example.org/onto/class/google_container_node_pool"/>
    <rdfs:range rdf:resource="http://www.w3.org/2001/XMLSchema#string"/>
  </owl:DatatypeProperty>
  <owl:DatatypeProperty rdf:about="http://example.org/onto/prop/google_container_node_pool_metadata">
    <rdfs:label>metadata</rdfs:label>
    <rdfs:comment>The metadata key/value pairs assigned to instances in the cluster.</rdfs:comment>
    <rdfs:domain rdf:resource="http://example.org/onto/class/google_container_node_pool"/>
    <rdfs:range rdf:resource="http://www.w3.org/2001/XMLSchema#string"/>
  </owl:DatatypeProperty>
  <owl:DatatypeProperty rdf:about="http://example.org/onto/prop/google_container_node_pool_min_cpu_platform">
    <rdfs:label>min_cpu_platform</rdfs:label>
    <rdfs:comment>Minimum CPU platform to be used by this instance. The instance may be scheduled on the specified or newer CPU platform.</rdfs:comment>
    <rdfs:domain rdf:resource="http://example.org/onto/class/google_container_node_pool"/>
    <rdfs:range rdf:resource="http://www.w3.org/2001/XMLSchema#string"/>
  </owl:DatatypeProperty>
  <owl:DatatypeProperty rdf:about="http://example.org/onto/prop/google_container_node_pool_node_group">
    <rdfs:label>node_group</rdfs:label>
    <rdfs:comment>Setting this field will assign instances of this pool to run on the specified node group. This is useful for running workloads on sole tenant nodes.</rdfs:comment>
    <rdfs:domain rdf:resource="http://example.org/onto/class/google_container_node_pool"/>
    <rdfs:range rdf:resource="http://www.w3.org/2001/XMLSchema#string"/>
  </owl:DatatypeProperty>
  <owl:DatatypeProperty rdf:about="http://example.org/onto/prop/google_container_node_pool_oauth_scopes">
    <rdfs:label>oauth_scopes</rdfs:label>
    <rdfs:comment>The set of Google API scopes to be made available on all of the node VMs.</rdfs:comment>
    <rdfs:domain rdf:resource="http://example.org/onto/class/google_container_node_pool"/>
    <rdfs:range rdf:resource="http://www.w3.org/2001/XMLSchema#string"/>
  </owl:DatatypeProperty>
  <owl:DatatypeProperty rdf:about="http://example.org/onto/prop/google_container_node_pool_preemptible">
    <rdfs:label>preemptible</rdfs:label>
    <rdfs:comment>Whether the nodes are created as preemptible VM instances.</rdfs:comment>
    <rdfs:domain rdf:resource="http://example.org/onto/class/google_container_node_pool"/>
    <rdfs:range rdf:resource="http://www.w3.org/2001/XMLSchema#string"/>
  </owl:DatatypeProperty>
  <owl:DatatypeProperty rdf:about="http://example.org/onto/prop/google_container_node_pool_resource_labels">
    <rdfs:label>resource_labels</rdfs:label>
    <rdfs:comment>The GCE resource labels (a map of key/value pairs) to be applied to the node pool.</rdfs:comment>
    <rdfs:domain rdf:resource="http://example.org/onto/class/google_container_node_pool"/>
    <rdfs:range rdf:resource="http://www.w3.org/2001/XMLSchema#string"/>
  </owl:DatatypeProperty>
  <owl:DatatypeProperty rdf:about="http://example.org/onto/prop/google_container_node_pool_resource_manager_tags">
    <rdfs:label>resource_manager_tags</rdfs:label>
    <rdfs:comment>A map of resource manager tags. Resource manager tag keys and values have the same definition as resource manager tags. Keys must be in the format tagKeys/{tag_key_id}, and values are in the format tagValues/456. The field is ignored (both PUT & PATCH) when empty.</rdfs:comment>
    <rdfs:domain rdf:resource="http://example.org/onto/class/google_container_node_pool"/>
    <rdfs:range rdf:resource="http://www.w3.org/2001/XMLSchema#string"/>
  </owl:DatatypeProperty>
  <owl:DatatypeProperty rdf:about="http://example.org/onto/prop/google_container_node_pool_service_account">
    <rdfs:label>service_account</rdfs:label>
    <rdfs:comment>The Google Cloud Platform Service Account to be used by the node VMs.</rdfs:comment>
    <rdfs:domain rdf:resource="http://example.org/onto/class/google_container_node_pool"/>
    <rdfs:range rdf:resource="http://www.w3.org/2001/XMLSchema#string"/>
  </owl:DatatypeProperty>
  <owl:DatatypeProperty rdf:about="http://example.org/onto/prop/google_container_node_pool_spot">
    <rdfs:label>spot</rdfs:label>
    <rdfs:comment>Whether the nodes are created as spot VM instances.</rdfs:comment>
    <rdfs:domain rdf:resource="http://example.org/onto/class/google_container_node_pool"/>
    <rdfs:range rdf:resource="http://www.w3.org/2001/XMLSchema#string"/>
  </owl:DatatypeProperty>
  <owl:DatatypeProperty rdf:about="http://example.org/onto/prop/google_container_node_pool_storage_pools">
    <rdfs:label>storage_pools</rdfs:label>
    <rdfs:comment>The list of Storage Pools where boot disks are provisioned.</rdfs:comment>
    <rdfs:domain rdf:resource="http://example.org/onto/class/google_container_node_pool"/>
    <rdfs:range rdf:resource="http://www.w3.org/2001/XMLSchema#string"/>
  </owl:DatatypeProperty>
  <owl:DatatypeProperty rdf:about="http://example.org/onto/prop/google_container_node_pool_tags">
    <rdfs:label>tags</rdfs:label>
    <rdfs:comment>The list of instance tags applied to all nodes.</rdfs:comment>
    <rdfs:domain rdf:resource="http://example.org/onto/class/google_container_node_pool"/>
    <rdfs:range rdf:resource="http://www.w3.org/2001/XMLSchema#string"/>
  </owl:DatatypeProperty>
  <owl:DatatypeProperty rdf:about="http://example.org/onto/prop/google_container_node_pool_enable_nested_virtualization">
    <rdfs:label>enable_nested_virtualization</rdfs:label>
    <rdfs:comment>Whether the node should have nested virtualization enabled.</rdfs:comment>
    <rdfs:domain rdf:resource="http://example.org/onto/class/google_container_node_pool"/>
    <rdfs:range rdf:resource="http://www.w3.org/2001/XMLSchema#string"/>
  </owl:DatatypeProperty>
  <owl:DatatypeProperty rdf:about="http://example.org/onto/prop/google_container_node_pool_performance_monitoring_unit">
    <rdfs:label>performance_monitoring_unit</rdfs:label>
    <rdfs:comment>Level of Performance Monitoring Unit (PMU) requested. If unset, no access to the PMU is assumed.</rdfs:comment>
    <rdfs:domain rdf:resource="http://example.org/onto/class/google_container_node_pool"/>
    <rdfs:range rdf:resource="http://www.w3.org/2001/XMLSchema#string"/>
  </owl:DatatypeProperty>
  <owl:DatatypeProperty rdf:about="http://example.org/onto/prop/google_container_node_pool_threads_per_core">
    <rdfs:label>threads_per_core</rdfs:label>
    <rdfs:comment>The number of threads per physical core. To disable simultaneous multithreading (SMT) set this to 1. If unset, the maximum number of threads supported per core by the underlying processor is assumed.</rdfs:comment>
    <rdfs:domain rdf:resource="http://example.org/onto/class/google_container_node_pool"/>
    <rdfs:range rdf:resource="http://www.w3.org/2001/XMLSchema#string"/>
  </owl:DatatypeProperty>
  <owl:DatatypeProperty rdf:about="http://example.org/onto/prop/google_container_node_pool_disk_type">
    <rdfs:label>disk_type</rdfs:label>
    <rdfs:comment>Type of the disk attached to each node. Such as pd-standard, pd-balanced or pd-ssd</rdfs:comment>
    <rdfs:domain rdf:resource="http://example.org/onto/class/google_container_node_pool"/>
    <rdfs:range rdf:resource="http://www.w3.org/2001/XMLSchema#string"/>
  </owl:DatatypeProperty>
  <owl:DatatypeProperty rdf:about="http://example.org/onto/prop/google_container_node_pool_provisioned_iops">
    <rdfs:label>provisioned_iops</rdfs:label>
    <rdfs:comment>Configured IOPs provisioning. Only valid with disk type hyperdisk-balanced.</rdfs:comment>
    <rdfs:domain rdf:resource="http://example.org/onto/class/google_container_node_pool"/>
    <rdfs:range rdf:resource="http://www.w3.org/2001/XMLSchema#string"/>
  </owl:DatatypeProperty>
  <owl:DatatypeProperty rdf:about="http://example.org/onto/prop/google_container_node_pool_provisioned_throughput">
    <rdfs:label>provisioned_throughput</rdfs:label>
    <rdfs:comment>Configured throughput provisioning. Only valid with disk type hyperdisk-balanced.</rdfs:comment>
    <rdfs:domain rdf:resource="http://example.org/onto/class/google_container_node_pool"/>
    <rdfs:range rdf:resource="http://www.w3.org/2001/XMLSchema#string"/>
  </owl:DatatypeProperty>
  <owl:DatatypeProperty rdf:about="http://example.org/onto/prop/google_container_node_pool_size_gb">
    <rdfs:label>size_gb</rdfs:label>
    <rdfs:comment>Size of the disk attached to each node, specified in GB. The smallest allowed disk size is 10GB.</rdfs:comment>
    <rdfs:domain rdf:resource="http://example.org/onto/class/google_container_node_pool"/>
    <rdfs:range rdf:resource="http://www.w3.org/2001/XMLSchema#string"/>
  </owl:DatatypeProperty>
  <owl:DatatypeProperty rdf:about="http://example.org/onto/prop/google_container_node_pool_confidential_instance_type">
    <rdfs:label>confidential_instance_type</rdfs:label>
    <rdfs:comment>Defines the type of technology used by the confidential node.</rdfs:comment>
    <rdfs:domain rdf:resource="http://example.org/onto/class/google_container_node_pool"/>
    <rdfs:range rdf:resource="http://www.w3.org/2001/XMLSchema#string"/>
  </owl:DatatypeProperty>
  <owl:DatatypeProperty rdf:about="http://example.org/onto/prop/google_container_node_pool_enabled">
    <rdfs:label>enabled</rdfs:label>
    <rdfs:comment>Whether Confidential Nodes feature is enabled for all nodes in this pool.</rdfs:comment>
    <rdfs:domain rdf:resource="http://example.org/onto/class/google_container_node_pool"/>
    <rdfs:range rdf:resource="http://www.w3.org/2001/XMLSchema#string"/>
  </owl:DatatypeProperty>
  <owl:DatatypeProperty rdf:about="http://example.org/onto/prop/google_container_node_pool_enabled">
    <rdfs:label>enabled</rdfs:label>
    <rdfs:comment>Whether or not private registries are configured.</rdfs:comment>
    <rdfs:domain rdf:resource="http://example.org/onto/class/google_container_node_pool"/>
    <rdfs:range rdf:resource="http://www.w3.org/2001/XMLSchema#string"/>
  </owl:DatatypeProperty>
  <owl:DatatypeProperty rdf:about="http://example.org/onto/prop/google_container_node_pool_fqdns">
    <rdfs:label>fqdns</rdfs:label>
    <rdfs:comment>List of fully-qualified-domain-names. IPv4s and port specification are supported.</rdfs:comment>
    <rdfs:domain rdf:resource="http://example.org/onto/class/google_container_node_pool"/>
    <rdfs:range rdf:resource="http://www.w3.org/2001/XMLSchema#string"/>
  </owl:DatatypeProperty>
  <owl:DatatypeProperty rdf:about="http://example.org/onto/prop/google_container_node_pool_secret_uri">
    <rdfs:label>secret_uri</rdfs:label>
    <rdfs:comment>URI for the secret that hosts a certificate. Must be in the format 'projects/PROJECT_NUM/secrets/SECRET_NAME/versions/VERSION_OR_LATEST'.</rdfs:comment>
    <rdfs:domain rdf:resource="http://example.org/onto/class/google_container_node_pool"/>
    <rdfs:range rdf:resource="http://www.w3.org/2001/XMLSchema#string"/>
  </owl:DatatypeProperty>
  <owl:DatatypeProperty rdf:about="http://example.org/onto/prop/google_container_node_pool_data_cache_count">
    <rdfs:label>data_cache_count</rdfs:label>
    <rdfs:comment>Number of local SSDs to be utilized for GKE Data Cache. Uses NVMe interfaces.</rdfs:comment>
    <rdfs:domain rdf:resource="http://example.org/onto/class/google_container_node_pool"/>
    <rdfs:range rdf:resource="http://www.w3.org/2001/XMLSchema#string"/>
  </owl:DatatypeProperty>
  <owl:DatatypeProperty rdf:about="http://example.org/onto/prop/google_container_node_pool_local_ssd_count">
    <rdfs:label>local_ssd_count</rdfs:label>
    <rdfs:comment>Number of local SSDs to use to back ephemeral storage. Uses NVMe interfaces. Each local SSD must be 375 or 3000 GB in size, and all local SSDs must share the same size.</rdfs:comment>
    <rdfs:domain rdf:resource="http://example.org/onto/class/google_container_node_pool"/>
    <rdfs:range rdf:resource="http://www.w3.org/2001/XMLSchema#string"/>
  </owl:DatatypeProperty>
  <owl:DatatypeProperty rdf:about="http://example.org/onto/prop/google_container_node_pool_enabled">
    <rdfs:label>enabled</rdfs:label>
    <rdfs:comment>Whether or not NCCL Fast Socket is enabled</rdfs:comment>
    <rdfs:domain rdf:resource="http://example.org/onto/class/google_container_node_pool"/>
    <rdfs:range rdf:resource="http://www.w3.org/2001/XMLSchema#string"/>
  </owl:DatatypeProperty>
  <owl:DatatypeProperty rdf:about="http://example.org/onto/prop/google_container_node_pool_enabled">
    <rdfs:label>enabled</rdfs:label>
    <rdfs:comment>Whether or not GCFS is enabled</rdfs:comment>
    <rdfs:domain rdf:resource="http://example.org/onto/class/google_container_node_pool"/>
    <rdfs:range rdf:resource="http://www.w3.org/2001/XMLSchema#string"/>
  </owl:DatatypeProperty>
  <owl:DatatypeProperty rdf:about="http://example.org/onto/prop/google_container_node_pool_count">
    <rdfs:label>count</rdfs:label>
    <rdfs:comment>The number of the accelerator cards exposed to an instance.</rdfs:comment>
    <rdfs:domain rdf:resource="http://example.org/onto/class/google_container_node_pool"/>
    <rdfs:range rdf:resource="http://www.w3.org/2001/XMLSchema#string"/>
  </owl:DatatypeProperty>
  <owl:DatatypeProperty rdf:about="http://example.org/onto/prop/google_container_node_pool_gpu_partition_size">
    <rdfs:label>gpu_partition_size</rdfs:label>
    <rdfs:comment>Size of partitions to create on the GPU. Valid values are described in the NVIDIA mig user guide (https://docs.nvidia.com/datacenter/tesla/mig-user-guide/#partitioning)</rdfs:comment>
    <rdfs:domain rdf:resource="http://example.org/onto/class/google_container_node_pool"/>
    <rdfs:range rdf:resource="http://www.w3.org/2001/XMLSchema#string"/>
  </owl:DatatypeProperty>
  <owl:DatatypeProperty rdf:about="http://example.org/onto/prop/google_container_node_pool_type">
    <rdfs:label>type</rdfs:label>
    <rdfs:comment>The accelerator type resource name.</rdfs:comment>
    <rdfs:domain rdf:resource="http://example.org/onto/class/google_container_node_pool"/>
    <rdfs:range rdf:resource="http://www.w3.org/2001/XMLSchema#string"/>
  </owl:DatatypeProperty>
  <owl:DatatypeProperty rdf:about="http://example.org/onto/prop/google_container_node_pool_gpu_driver_version">
    <rdfs:label>gpu_driver_version</rdfs:label>
    <rdfs:comment>Mode for how the GPU driver is installed.</rdfs:comment>
    <rdfs:domain rdf:resource="http://example.org/onto/class/google_container_node_pool"/>
    <rdfs:range rdf:resource="http://www.w3.org/2001/XMLSchema#string"/>
  </owl:DatatypeProperty>
  <owl:DatatypeProperty rdf:about="http://example.org/onto/prop/google_container_node_pool_gpu_sharing_strategy">
    <rdfs:label>gpu_sharing_strategy</rdfs:label>
    <rdfs:comment>The type of GPU sharing strategy to enable on the GPU node. Possible values are described in the API package (https://pkg.go.dev/google.golang.org/api/container/v1#GPUSharingConfig)</rdfs:comment>
    <rdfs:domain rdf:resource="http://example.org/onto/class/google_container_node_pool"/>
    <rdfs:range rdf:resource="http://www.w3.org/2001/XMLSchema#string"/>
  </owl:DatatypeProperty>
  <owl:DatatypeProperty rdf:about="http://example.org/onto/prop/google_container_node_pool_max_shared_clients_per_gpu">
    <rdfs:label>max_shared_clients_per_gpu</rdfs:label>
    <rdfs:comment>The maximum number of containers that can share a GPU.</rdfs:comment>
    <rdfs:domain rdf:resource="http://example.org/onto/class/google_container_node_pool"/>
    <rdfs:range rdf:resource="http://www.w3.org/2001/XMLSchema#string"/>
  </owl:DatatypeProperty>
  <owl:DatatypeProperty rdf:about="http://example.org/onto/prop/google_container_node_pool_enabled">
    <rdfs:label>enabled</rdfs:label>
    <rdfs:comment>Whether or not gvnic is enabled</rdfs:comment>
    <rdfs:domain rdf:resource="http://example.org/onto/class/google_container_node_pool"/>
    <rdfs:range rdf:resource="http://www.w3.org/2001/XMLSchema#string"/>
  </owl:DatatypeProperty>
  <owl:DatatypeProperty rdf:about="http://example.org/onto/prop/google_container_node_pool_maintenance_interval">
    <rdfs:label>maintenance_interval</rdfs:label>
    <rdfs:comment>.</rdfs:comment>
    <rdfs:domain rdf:resource="http://example.org/onto/class/google_container_node_pool"/>
    <rdfs:range rdf:resource="http://www.w3.org/2001/XMLSchema#string"/>
  </owl:DatatypeProperty>
  <owl:DatatypeProperty rdf:about="http://example.org/onto/prop/google_container_node_pool_allowed_unsafe_sysctls">
    <rdfs:label>allowed_unsafe_sysctls</rdfs:label>
    <rdfs:comment>Defines a comma-separated allowlist of unsafe sysctls or sysctl patterns which can be set on the Pods.</rdfs:comment>
    <rdfs:domain rdf:resource="http://example.org/onto/class/google_container_node_pool"/>
    <rdfs:range rdf:resource="http://www.w3.org/2001/XMLSchema#string"/>
  </owl:DatatypeProperty>
  <owl:DatatypeProperty rdf:about="http://example.org/onto/prop/google_container_node_pool_container_log_max_files">
    <rdfs:label>container_log_max_files</rdfs:label>
    <rdfs:comment>Defines the maximum number of container log files that can be present for a container.</rdfs:comment>
    <rdfs:domain rdf:resource="http://example.org/onto/class/google_container_node_pool"/>
    <rdfs:range rdf:resource="http://www.w3.org/2001/XMLSchema#string"/>
  </owl:DatatypeProperty>
  <owl:DatatypeProperty rdf:about="http://example.org/onto/prop/google_container_node_pool_container_log_max_size">
    <rdfs:label>container_log_max_size</rdfs:label>
    <rdfs:comment>Defines the maximum size of the container log file before it is rotated.</rdfs:comment>
    <rdfs:domain rdf:resource="http://example.org/onto/class/google_container_node_pool"/>
    <rdfs:range rdf:resource="http://www.w3.org/2001/XMLSchema#string"/>
  </owl:DatatypeProperty>
  <owl:DatatypeProperty rdf:about="http://example.org/onto/prop/google_container_node_pool_cpu_cfs_quota">
    <rdfs:label>cpu_cfs_quota</rdfs:label>
    <rdfs:comment>Enable CPU CFS quota enforcement for containers that specify CPU limits.</rdfs:comment>
    <rdfs:domain rdf:resource="http://example.org/onto/class/google_container_node_pool"/>
    <rdfs:range rdf:resource="http://www.w3.org/2001/XMLSchema#string"/>
  </owl:DatatypeProperty>
  <owl:DatatypeProperty rdf:about="http://example.org/onto/prop/google_container_node_pool_cpu_cfs_quota_period">
    <rdfs:label>cpu_cfs_quota_period</rdfs:label>
    <rdfs:comment>Set the CPU CFS quota period value 'cpu.cfs_period_us'.</rdfs:comment>
    <rdfs:domain rdf:resource="http://example.org/onto/class/google_container_node_pool"/>
    <rdfs:range rdf:resource="http://www.w3.org/2001/XMLSchema#string"/>
  </owl:DatatypeProperty>
  <owl:DatatypeProperty rdf:about="http://example.org/onto/prop/google_container_node_pool_cpu_manager_policy">
    <rdfs:label>cpu_manager_policy</rdfs:label>
    <rdfs:comment>Control the CPU management policy on the node.</rdfs:comment>
    <rdfs:domain rdf:resource="http://example.org/onto/class/google_container_node_pool"/>
    <rdfs:range rdf:resource="http://www.w3.org/2001/XMLSchema#string"/>
  </owl:DatatypeProperty>
  <owl:DatatypeProperty rdf:about="http://example.org/onto/prop/google_container_node_pool_eviction_max_pod_grace_period_seconds">
    <rdfs:label>eviction_max_pod_grace_period_seconds</rdfs:label>
    <rdfs:comment>Defines the maximum allowed grace period (in seconds) to use when terminating pods in response to a soft eviction threshold being met.</rdfs:comment>
    <rdfs:domain rdf:resource="http://example.org/onto/class/google_container_node_pool"/>
    <rdfs:range rdf:resource="http://www.w3.org/2001/XMLSchema#string"/>
  </owl:DatatypeProperty>
  <owl:DatatypeProperty rdf:about="http://example.org/onto/prop/google_container_node_pool_image_gc_high_threshold_percent">
    <rdfs:label>image_gc_high_threshold_percent</rdfs:label>
    <rdfs:comment>Defines the percent of disk usage after which image garbage collection is always run.</rdfs:comment>
    <rdfs:domain rdf:resource="http://example.org/onto/class/google_container_node_pool"/>
    <rdfs:range rdf:resource="http://www.w3.org/2001/XMLSchema#string"/>
  </owl:DatatypeProperty>
  <owl:DatatypeProperty rdf:about="http://example.org/onto/prop/google_container_node_pool_image_gc_low_threshold_percent">
    <rdfs:label>image_gc_low_threshold_percent</rdfs:label>
    <rdfs:comment>Defines the percent of disk usage before which image garbage collection is never run. Lowest disk usage to garbage collect to.</rdfs:comment>
    <rdfs:domain rdf:resource="http://example.org/onto/class/google_container_node_pool"/>
    <rdfs:range rdf:resource="http://www.w3.org/2001/XMLSchema#string"/>
  </owl:DatatypeProperty>
  <owl:DatatypeProperty rdf:about="http://example.org/onto/prop/google_container_node_pool_image_maximum_gc_age">
    <rdfs:label>image_maximum_gc_age</rdfs:label>
    <rdfs:comment>Defines the maximum age an image can be unused before it is garbage collected.</rdfs:comment>
    <rdfs:domain rdf:resource="http://example.org/onto/class/google_container_node_pool"/>
    <rdfs:range rdf:resource="http://www.w3.org/2001/XMLSchema#string"/>
  </owl:DatatypeProperty>
  <owl:DatatypeProperty rdf:about="http://example.org/onto/prop/google_container_node_pool_image_minimum_gc_age">
    <rdfs:label>image_minimum_gc_age</rdfs:label>
    <rdfs:comment>Defines the minimum age for an unused image before it is garbage collected.</rdfs:comment>
    <rdfs:domain rdf:resource="http://example.org/onto/class/google_container_node_pool"/>
    <rdfs:range rdf:resource="http://www.w3.org/2001/XMLSchema#string"/>
  </owl:DatatypeProperty>
  <owl:DatatypeProperty rdf:about="http://example.org/onto/prop/google_container_node_pool_insecure_kubelet_readonly_port_enabled">
    <rdfs:label>insecure_kubelet_readonly_port_enabled</rdfs:label>
    <rdfs:comment>Controls whether the kubelet read-only port is enabled. It is strongly recommended to set this to `FALSE`. Possible values: `TRUE`, `FALSE`.</rdfs:comment>
    <rdfs:domain rdf:resource="http://example.org/onto/class/google_container_node_pool"/>
    <rdfs:range rdf:resource="http://www.w3.org/2001/XMLSchema#string"/>
  </owl:DatatypeProperty>
  <owl:DatatypeProperty rdf:about="http://example.org/onto/prop/google_container_node_pool_max_parallel_image_pulls">
    <rdfs:label>max_parallel_image_pulls</rdfs:label>
    <rdfs:comment>Set the maximum number of image pulls in parallel.</rdfs:comment>
    <rdfs:domain rdf:resource="http://example.org/onto/class/google_container_node_pool"/>
    <rdfs:range rdf:resource="http://www.w3.org/2001/XMLSchema#string"/>
  </owl:DatatypeProperty>
  <owl:DatatypeProperty rdf:about="http://example.org/onto/prop/google_container_node_pool_pod_pids_limit">
    <rdfs:label>pod_pids_limit</rdfs:label>
    <rdfs:comment>Controls the maximum number of processes allowed to run in a pod.</rdfs:comment>
    <rdfs:domain rdf:resource="http://example.org/onto/class/google_container_node_pool"/>
    <rdfs:range rdf:resource="http://www.w3.org/2001/XMLSchema#string"/>
  </owl:DatatypeProperty>
  <owl:DatatypeProperty rdf:about="http://example.org/onto/prop/google_container_node_pool_single_process_oom_kill">
    <rdfs:label>single_process_oom_kill</rdfs:label>
    <rdfs:comment>Defines whether to enable single process OOM killer.</rdfs:comment>
    <rdfs:domain rdf:resource="http://example.org/onto/class/google_container_node_pool"/>
    <rdfs:range rdf:resource="http://www.w3.org/2001/XMLSchema#string"/>
  </owl:DatatypeProperty>
  <owl:DatatypeProperty rdf:about="http://example.org/onto/prop/google_container_node_pool_imagefs_available">
    <rdfs:label>imagefs_available</rdfs:label>
    <rdfs:comment>Defines percentage of minimum reclaim for imagefs.available.</rdfs:comment>
    <rdfs:domain rdf:resource="http://example.org/onto/class/google_container_node_pool"/>
    <rdfs:range rdf:resource="http://www.w3.org/2001/XMLSchema#string"/>
  </owl:DatatypeProperty>
  <owl:DatatypeProperty rdf:about="http://example.org/onto/prop/google_container_node_pool_imagefs_inodes_free">
    <rdfs:label>imagefs_inodes_free</rdfs:label>
    <rdfs:comment>Defines percentage of minimum reclaim for imagefs.inodesFree.</rdfs:comment>
    <rdfs:domain rdf:resource="http://example.org/onto/class/google_container_node_pool"/>
    <rdfs:range rdf:resource="http://www.w3.org/2001/XMLSchema#string"/>
  </owl:DatatypeProperty>
  <owl:DatatypeProperty rdf:about="http://example.org/onto/prop/google_container_node_pool_memory_available">
    <rdfs:label>memory_available</rdfs:label>
    <rdfs:comment>Defines percentage of minimum reclaim for memory.available.</rdfs:comment>
    <rdfs:domain rdf:resource="http://example.org/onto/class/google_container_node_pool"/>
    <rdfs:range rdf:resource="http://www.w3.org/2001/XMLSchema#string"/>
  </owl:DatatypeProperty>
  <owl:DatatypeProperty rdf:about="http://example.org/onto/prop/google_container_node_pool_nodefs_available">
    <rdfs:label>nodefs_available</rdfs:label>
    <rdfs:comment>Defines percentage of minimum reclaim for nodefs.available.</rdfs:comment>
    <rdfs:domain rdf:resource="http://example.org/onto/class/google_container_node_pool"/>
    <rdfs:range rdf:resource="http://www.w3.org/2001/XMLSchema#string"/>
  </owl:DatatypeProperty>
  <owl:DatatypeProperty rdf:about="http://example.org/onto/prop/google_container_node_pool_nodefs_inodes_free">
    <rdfs:label>nodefs_inodes_free</rdfs:label>
    <rdfs:comment>Defines percentage of minimum reclaim for nodefs.inodesFree.</rdfs:comment>
    <rdfs:domain rdf:resource="http://example.org/onto/class/google_container_node_pool"/>
    <rdfs:range rdf:resource="http://www.w3.org/2001/XMLSchema#string"/>
  </owl:DatatypeProperty>
  <owl:DatatypeProperty rdf:about="http://example.org/onto/prop/google_container_node_pool_pid_available">
    <rdfs:label>pid_available</rdfs:label>
    <rdfs:comment>Defines percentage of minimum reclaim for pid.available.</rdfs:comment>
    <rdfs:domain rdf:resource="http://example.org/onto/class/google_container_node_pool"/>
    <rdfs:range rdf:resource="http://www.w3.org/2001/XMLSchema#string"/>
  </owl:DatatypeProperty>
  <owl:DatatypeProperty rdf:about="http://example.org/onto/prop/google_container_node_pool_imagefs_available">
    <rdfs:label>imagefs_available</rdfs:label>
    <rdfs:comment>Defines percentage of soft eviction threshold for imagefs.available.</rdfs:comment>
    <rdfs:domain rdf:resource="http://example.org/onto/class/google_container_node_pool"/>
    <rdfs:range rdf:resource="http://www.w3.org/2001/XMLSchema#string"/>
  </owl:DatatypeProperty>
  <owl:DatatypeProperty rdf:about="http://example.org/onto/prop/google_container_node_pool_imagefs_inodes_free">
    <rdfs:label>imagefs_inodes_free</rdfs:label>
    <rdfs:comment>Defines percentage of soft eviction threshold for imagefs.inodesFree.</rdfs:comment>
    <rdfs:domain rdf:resource="http://example.org/onto/class/google_container_node_pool"/>
    <rdfs:range rdf:resource="http://www.w3.org/2001/XMLSchema#string"/>
  </owl:DatatypeProperty>
  <owl:DatatypeProperty rdf:about="http://example.org/onto/prop/google_container_node_pool_memory_available">
    <rdfs:label>memory_available</rdfs:label>
    <rdfs:comment>Defines quantity of soft eviction threshold for memory.available.</rdfs:comment>
    <rdfs:domain rdf:resource="http://example.org/onto/class/google_container_node_pool"/>
    <rdfs:range rdf:resource="http://www.w3.org/2001/XMLSchema#string"/>
  </owl:DatatypeProperty>
  <owl:DatatypeProperty rdf:about="http://example.org/onto/prop/google_container_node_pool_nodefs_available">
    <rdfs:label>nodefs_available</rdfs:label>
    <rdfs:comment>Defines percentage of soft eviction threshold for nodefs.available.</rdfs:comment>
    <rdfs:domain rdf:resource="http://example.org/onto/class/google_container_node_pool"/>
    <rdfs:range rdf:resource="http://www.w3.org/2001/XMLSchema#string"/>
  </owl:DatatypeProperty>
  <owl:DatatypeProperty rdf:about="http://example.org/onto/prop/google_container_node_pool_nodefs_inodes_free">
    <rdfs:label>nodefs_inodes_free</rdfs:label>
    <rdfs:comment>Defines percentage of soft eviction threshold for nodefs.inodesFree.</rdfs:comment>
    <rdfs:domain rdf:resource="http://example.org/onto/class/google_container_node_pool"/>
    <rdfs:range rdf:resource="http://www.w3.org/2001/XMLSchema#string"/>
  </owl:DatatypeProperty>
  <owl:DatatypeProperty rdf:about="http://example.org/onto/prop/google_container_node_pool_pid_available">
    <rdfs:label>pid_available</rdfs:label>
    <rdfs:comment>Defines percentage of soft eviction threshold for pid.available.</rdfs:comment>
    <rdfs:domain rdf:resource="http://example.org/onto/class/google_container_node_pool"/>
    <rdfs:range rdf:resource="http://www.w3.org/2001/XMLSchema#string"/>
  </owl:DatatypeProperty>
  <owl:DatatypeProperty rdf:about="http://example.org/onto/prop/google_container_node_pool_imagefs_available">
    <rdfs:label>imagefs_available</rdfs:label>
    <rdfs:comment>Defines grace period for the imagefs.available soft eviction threshold</rdfs:comment>
    <rdfs:domain rdf:resource="http://example.org/onto/class/google_container_node_pool"/>
    <rdfs:range rdf:resource="http://www.w3.org/2001/XMLSchema#string"/>
  </owl:DatatypeProperty>
  <owl:DatatypeProperty rdf:about="http://example.org/onto/prop/google_container_node_pool_imagefs_inodes_free">
    <rdfs:label>imagefs_inodes_free</rdfs:label>
    <rdfs:comment>Defines grace period for the imagefs.inodesFree soft eviction threshold.</rdfs:comment>
    <rdfs:domain rdf:resource="http://example.org/onto/class/google_container_node_pool"/>
    <rdfs:range rdf:resource="http://www.w3.org/2001/XMLSchema#string"/>
  </owl:DatatypeProperty>
  <owl:DatatypeProperty rdf:about="http://example.org/onto/prop/google_container_node_pool_memory_available">
    <rdfs:label>memory_available</rdfs:label>
    <rdfs:comment>Defines grace period for the memory.available soft eviction threshold.</rdfs:comment>
    <rdfs:domain rdf:resource="http://example.org/onto/class/google_container_node_pool"/>
    <rdfs:range rdf:resource="http://www.w3.org/2001/XMLSchema#string"/>
  </owl:DatatypeProperty>
  <owl:DatatypeProperty rdf:about="http://example.org/onto/prop/google_container_node_pool_nodefs_available">
    <rdfs:label>nodefs_available</rdfs:label>
    <rdfs:comment>Defines grace period for the nodefs.available soft eviction threshold.</rdfs:comment>
    <rdfs:domain rdf:resource="http://example.org/onto/class/google_container_node_pool"/>
    <rdfs:range rdf:resource="http://www.w3.org/2001/XMLSchema#string"/>
  </owl:DatatypeProperty>
  <owl:DatatypeProperty rdf:about="http://example.org/onto/prop/google_container_node_pool_nodefs_inodes_free">
    <rdfs:label>nodefs_inodes_free</rdfs:label>
    <rdfs:comment>Defines grace period for the nodefs.inodesFree soft eviction threshold.</rdfs:comment>
    <rdfs:domain rdf:resource="http://example.org/onto/class/google_container_node_pool"/>
    <rdfs:range rdf:resource="http://www.w3.org/2001/XMLSchema#string"/>
  </owl:DatatypeProperty>
  <owl:DatatypeProperty rdf:about="http://example.org/onto/prop/google_container_node_pool_pid_available">
    <rdfs:label>pid_available</rdfs:label>
    <rdfs:comment>Defines grace period for the pid.available soft eviction threshold.</rdfs:comment>
    <rdfs:domain rdf:resource="http://example.org/onto/class/google_container_node_pool"/>
    <rdfs:range rdf:resource="http://www.w3.org/2001/XMLSchema#string"/>
  </owl:DatatypeProperty>
  <owl:DatatypeProperty rdf:about="http://example.org/onto/prop/google_container_node_pool_policy">
    <rdfs:label>policy</rdfs:label>
    <rdfs:comment>The Memory Manager policy to use. This policy guides how memory and hugepages are allocated and managed for pods on the node, influencing NUMA affinity.</rdfs:comment>
    <rdfs:domain rdf:resource="http://example.org/onto/class/google_container_node_pool"/>
    <rdfs:range rdf:resource="http://www.w3.org/2001/XMLSchema#string"/>
  </owl:DatatypeProperty>
  <owl:DatatypeProperty rdf:about="http://example.org/onto/prop/google_container_node_pool_policy">
    <rdfs:label>policy</rdfs:label>
    <rdfs:comment>The Topology Manager policy to use. This policy dictates how resource alignment is handled on the node.</rdfs:comment>
    <rdfs:domain rdf:resource="http://example.org/onto/class/google_container_node_pool"/>
    <rdfs:range rdf:resource="http://www.w3.org/2001/XMLSchema#string"/>
  </owl:DatatypeProperty>
  <owl:DatatypeProperty rdf:about="http://example.org/onto/prop/google_container_node_pool_scope">
    <rdfs:label>scope</rdfs:label>
    <rdfs:comment>The Topology Manager scope, defining the granularity at which policy decisions are applied. Valid values are "container" (resources are aligned per container within a pod) or "pod" (resources are aligned for the entire pod).</rdfs:comment>
    <rdfs:domain rdf:resource="http://example.org/onto/class/google_container_node_pool"/>
    <rdfs:range rdf:resource="http://www.w3.org/2001/XMLSchema#string"/>
  </owl:DatatypeProperty>
  <owl:DatatypeProperty rdf:about="http://example.org/onto/prop/google_container_node_pool_cgroup_mode">
    <rdfs:label>cgroup_mode</rdfs:label>
    <rdfs:comment>cgroupMode specifies the cgroup mode to be used on the node.</rdfs:comment>
    <rdfs:domain rdf:resource="http://example.org/onto/class/google_container_node_pool"/>
    <rdfs:range rdf:resource="http://www.w3.org/2001/XMLSchema#string"/>
  </owl:DatatypeProperty>
  <owl:DatatypeProperty rdf:about="http://example.org/onto/prop/google_container_node_pool_sysctls">
    <rdfs:label>sysctls</rdfs:label>
    <rdfs:comment>The Linux kernel parameters to be applied to the nodes and all pods running on the nodes.</rdfs:comment>
    <rdfs:domain rdf:resource="http://example.org/onto/class/google_container_node_pool"/>
    <rdfs:range rdf:resource="http://www.w3.org/2001/XMLSchema#string"/>
  </owl:DatatypeProperty>
  <owl:DatatypeProperty rdf:about="http://example.org/onto/prop/google_container_node_pool_transparent_hugepage_defrag">
    <rdfs:label>transparent_hugepage_defrag</rdfs:label>
    <rdfs:comment>The Linux kernel transparent hugepage defrag setting.</rdfs:comment>
    <rdfs:domain rdf:resource="http://example.org/onto/class/google_container_node_pool"/>
    <rdfs:range rdf:resource="http://www.w3.org/2001/XMLSchema#string"/>
  </owl:DatatypeProperty>
  <owl:DatatypeProperty rdf:about="http://example.org/onto/prop/google_container_node_pool_transparent_hugepage_enabled">
    <rdfs:label>transparent_hugepage_enabled</rdfs:label>
    <rdfs:comment>The Linux kernel transparent hugepage setting.</rdfs:comment>
    <rdfs:domain rdf:resource="http://example.org/onto/class/google_container_node_pool"/>
    <rdfs:range rdf:resource="http://www.w3.org/2001/XMLSchema#string"/>
  </owl:DatatypeProperty>
  <owl:DatatypeProperty rdf:about="http://example.org/onto/prop/google_container_node_pool_hugepage_size_1g">
    <rdfs:label>hugepage_size_1g</rdfs:label>
    <rdfs:comment>Amount of 1G hugepages.</rdfs:comment>
    <rdfs:domain rdf:resource="http://example.org/onto/class/google_container_node_pool"/>
    <rdfs:range rdf:resource="http://www.w3.org/2001/XMLSchema#string"/>
  </owl:DatatypeProperty>
  <owl:DatatypeProperty rdf:about="http://example.org/onto/prop/google_container_node_pool_hugepage_size_2m">
    <rdfs:label>hugepage_size_2m</rdfs:label>
    <rdfs:comment>Amount of 2M hugepages.</rdfs:comment>
    <rdfs:domain rdf:resource="http://example.org/onto/class/google_container_node_pool"/>
    <rdfs:range rdf:resource="http://www.w3.org/2001/XMLSchema#string"/>
  </owl:DatatypeProperty>
  <owl:DatatypeProperty rdf:about="http://example.org/onto/prop/google_container_node_pool_local_ssd_count">
    <rdfs:label>local_ssd_count</rdfs:label>
    <rdfs:comment>Number of raw-block local NVMe SSD disks to be attached to the node. Each local SSD is 375 GB in size.</rdfs:comment>
    <rdfs:domain rdf:resource="http://example.org/onto/class/google_container_node_pool"/>
    <rdfs:range rdf:resource="http://www.w3.org/2001/XMLSchema#string"/>
  </owl:DatatypeProperty>
  <owl:DatatypeProperty rdf:about="http://example.org/onto/prop/google_container_node_pool_consume_reservation_type">
    <rdfs:label>consume_reservation_type</rdfs:label>
    <rdfs:comment>Corresponds to the type of reservation consumption.</rdfs:comment>
    <rdfs:domain rdf:resource="http://example.org/onto/class/google_container_node_pool"/>
    <rdfs:range rdf:resource="http://www.w3.org/2001/XMLSchema#string"/>
  </owl:DatatypeProperty>
  <owl:DatatypeProperty rdf:about="http://example.org/onto/prop/google_container_node_pool_key">
    <rdfs:label>key</rdfs:label>
    <rdfs:comment>The label key of a reservation resource.</rdfs:comment>
    <rdfs:domain rdf:resource="http://example.org/onto/class/google_container_node_pool"/>
    <rdfs:range rdf:resource="http://www.w3.org/2001/XMLSchema#string"/>
  </owl:DatatypeProperty>
  <owl:DatatypeProperty rdf:about="http://example.org/onto/prop/google_container_node_pool_values">
    <rdfs:label>values</rdfs:label>
    <rdfs:comment>The label values of the reservation resource.</rdfs:comment>
    <rdfs:domain rdf:resource="http://example.org/onto/class/google_container_node_pool"/>
    <rdfs:range rdf:resource="http://www.w3.org/2001/XMLSchema#string"/>
  </owl:DatatypeProperty>
  <owl:DatatypeProperty rdf:about="http://example.org/onto/prop/google_container_node_pool_disk_image">
    <rdfs:label>disk_image</rdfs:label>
    <rdfs:comment>Disk image to create the secondary boot disk from</rdfs:comment>
    <rdfs:domain rdf:resource="http://example.org/onto/class/google_container_node_pool"/>
    <rdfs:range rdf:resource="http://www.w3.org/2001/XMLSchema#string"/>
  </owl:DatatypeProperty>
  <owl:DatatypeProperty rdf:about="http://example.org/onto/prop/google_container_node_pool_mode">
    <rdfs:label>mode</rdfs:label>
    <rdfs:comment>Mode for how the secondary boot disk is used.</rdfs:comment>
    <rdfs:domain rdf:resource="http://example.org/onto/class/google_container_node_pool"/>
    <rdfs:range rdf:resource="http://www.w3.org/2001/XMLSchema#string"/>
  </owl:DatatypeProperty>
  <owl:DatatypeProperty rdf:about="http://example.org/onto/prop/google_container_node_pool_enable_integrity_monitoring">
    <rdfs:label>enable_integrity_monitoring</rdfs:label>
    <rdfs:comment>Defines whether the instance has integrity monitoring enabled.</rdfs:comment>
    <rdfs:domain rdf:resource="http://example.org/onto/class/google_container_node_pool"/>
    <rdfs:range rdf:resource="http://www.w3.org/2001/XMLSchema#string"/>
  </owl:DatatypeProperty>
  <owl:DatatypeProperty rdf:about="http://example.org/onto/prop/google_container_node_pool_enable_secure_boot">
    <rdfs:label>enable_secure_boot</rdfs:label>
    <rdfs:comment>Defines whether the instance has Secure Boot enabled.</rdfs:comment>
    <rdfs:domain rdf:resource="http://example.org/onto/class/google_container_node_pool"/>
    <rdfs:range rdf:resource="http://www.w3.org/2001/XMLSchema#string"/>
  </owl:DatatypeProperty>
  <owl:DatatypeProperty rdf:about="http://example.org/onto/prop/google_container_node_pool_min_node_cpus">
    <rdfs:label>min_node_cpus</rdfs:label>
    <rdfs:comment>Specifies the minimum number of vCPUs that each sole tenant node must have to use CPU overcommit. If not specified, the CPU overcommit feature is disabled.</rdfs:comment>
    <rdfs:domain rdf:resource="http://example.org/onto/class/google_container_node_pool"/>
    <rdfs:range rdf:resource="http://www.w3.org/2001/XMLSchema#string"/>
  </owl:DatatypeProperty>
  <owl:DatatypeProperty rdf:about="http://example.org/onto/prop/google_container_node_pool_key">
    <rdfs:label>key</rdfs:label>
    <rdfs:comment>.</rdfs:comment>
    <rdfs:domain rdf:resource="http://example.org/onto/class/google_container_node_pool"/>
    <rdfs:range rdf:resource="http://www.w3.org/2001/XMLSchema#string"/>
  </owl:DatatypeProperty>
  <owl:DatatypeProperty rdf:about="http://example.org/onto/prop/google_container_node_pool_operator">
    <rdfs:label>operator</rdfs:label>
    <rdfs:comment>.</rdfs:comment>
    <rdfs:domain rdf:resource="http://example.org/onto/class/google_container_node_pool"/>
    <rdfs:range rdf:resource="http://www.w3.org/2001/XMLSchema#string"/>
  </owl:DatatypeProperty>
  <owl:DatatypeProperty rdf:about="http://example.org/onto/prop/google_container_node_pool_values">
    <rdfs:label>values</rdfs:label>
    <rdfs:comment>.</rdfs:comment>
    <rdfs:domain rdf:resource="http://example.org/onto/class/google_container_node_pool"/>
    <rdfs:range rdf:resource="http://www.w3.org/2001/XMLSchema#string"/>
  </owl:DatatypeProperty>
  <owl:DatatypeProperty rdf:about="http://example.org/onto/prop/google_container_node_pool_effect">
    <rdfs:label>effect</rdfs:label>
    <rdfs:comment>Effect for taint.</rdfs:comment>
    <rdfs:domain rdf:resource="http://example.org/onto/class/google_container_node_pool"/>
    <rdfs:range rdf:resource="http://www.w3.org/2001/XMLSchema#string"/>
  </owl:DatatypeProperty>
  <owl:DatatypeProperty rdf:about="http://example.org/onto/prop/google_container_node_pool_key">
    <rdfs:label>key</rdfs:label>
    <rdfs:comment>Key for taint.</rdfs:comment>
    <rdfs:domain rdf:resource="http://example.org/onto/class/google_container_node_pool"/>
    <rdfs:range rdf:resource="http://www.w3.org/2001/XMLSchema#string"/>
  </owl:DatatypeProperty>
  <owl:DatatypeProperty rdf:about="http://example.org/onto/prop/google_container_node_pool_value">
    <rdfs:label>value</rdfs:label>
    <rdfs:comment>Value for taint.</rdfs:comment>
    <rdfs:domain rdf:resource="http://example.org/onto/class/google_container_node_pool"/>
    <rdfs:range rdf:resource="http://www.w3.org/2001/XMLSchema#string"/>
  </owl:DatatypeProperty>
  <owl:DatatypeProperty rdf:about="http://example.org/onto/prop/google_container_node_pool_osversion">
    <rdfs:label>osversion</rdfs:label>
    <rdfs:comment>The OS Version of the windows nodepool.Values are OS_VERSION_UNSPECIFIED,OS_VERSION_LTSC2019 and OS_VERSION_LTSC2022</rdfs:comment>
    <rdfs:domain rdf:resource="http://example.org/onto/class/google_container_node_pool"/>
    <rdfs:range rdf:resource="http://www.w3.org/2001/XMLSchema#string"/>
  </owl:DatatypeProperty>
  <owl:DatatypeProperty rdf:about="http://example.org/onto/prop/google_container_node_pool_mode">
    <rdfs:label>mode</rdfs:label>
    <rdfs:comment>Mode is the configuration for how to expose metadata to workloads running on the node.</rdfs:comment>
    <rdfs:domain rdf:resource="http://example.org/onto/class/google_container_node_pool"/>
    <rdfs:range rdf:resource="http://www.w3.org/2001/XMLSchema#string"/>
  </owl:DatatypeProperty>
  <owl:DatatypeProperty rdf:about="http://example.org/onto/prop/google_container_node_pool_policy_name">
    <rdfs:label>policy_name</rdfs:label>
    <rdfs:comment>If set, refers to the name of a custom resource policy supplied by the user. The resource policy must be in the same project and region as the node pool. If not found, InvalidArgument error is returned.</rdfs:comment>
    <rdfs:domain rdf:resource="http://example.org/onto/class/google_container_node_pool"/>
    <rdfs:range rdf:resource="http://www.w3.org/2001/XMLSchema#string"/>
  </owl:DatatypeProperty>
  <owl:DatatypeProperty rdf:about="http://example.org/onto/prop/google_container_node_pool_tpu_topology">
    <rdfs:label>tpu_topology</rdfs:label>
    <rdfs:comment>The TPU topology like "2x4" or "2x2x2". https://cloud.google.com/kubernetes-engine/docs/concepts/plan-tpus#topology</rdfs:comment>
    <rdfs:domain rdf:resource="http://example.org/onto/class/google_container_node_pool"/>
    <rdfs:range rdf:resource="http://www.w3.org/2001/XMLSchema#string"/>
  </owl:DatatypeProperty>
  <owl:DatatypeProperty rdf:about="http://example.org/onto/prop/google_container_node_pool_type">
    <rdfs:label>type</rdfs:label>
    <rdfs:comment>Type defines the type of placement policy</rdfs:comment>
    <rdfs:domain rdf:resource="http://example.org/onto/class/google_container_node_pool"/>
    <rdfs:range rdf:resource="http://www.w3.org/2001/XMLSchema#string"/>
  </owl:DatatypeProperty>
  <owl:DatatypeProperty rdf:about="http://example.org/onto/prop/google_container_node_pool_enabled">
    <rdfs:label>enabled</rdfs:label>
    <rdfs:comment>Whether nodes in this node pool are obtainable solely through the ProvisioningRequest API</rdfs:comment>
    <rdfs:domain rdf:resource="http://example.org/onto/class/google_container_node_pool"/>
    <rdfs:range rdf:resource="http://www.w3.org/2001/XMLSchema#string"/>
  </owl:DatatypeProperty>
  <owl:DatatypeProperty rdf:about="http://example.org/onto/prop/google_container_node_pool_create">
    <rdfs:label>create</rdfs:label>
    <rdfs:domain rdf:resource="http://example.org/onto/class/google_container_node_pool"/>
    <rdfs:range rdf:resource="http://www.w3.org/2001/XMLSchema#string"/>
  </owl:DatatypeProperty>
  <owl:DatatypeProperty rdf:about="http://example.org/onto/prop/google_container_node_pool_delete">
    <rdfs:label>delete</rdfs:label>
    <rdfs:domain rdf:resource="http://example.org/onto/class/google_container_node_pool"/>
    <rdfs:range rdf:resource="http://www.w3.org/2001/XMLSchema#string"/>
  </owl:DatatypeProperty>
  <owl:DatatypeProperty rdf:about="http://example.org/onto/prop/google_container_node_pool_update">
    <rdfs:label>update</rdfs:label>
    <rdfs:domain rdf:resource="http://example.org/onto/class/google_container_node_pool"/>
    <rdfs:range rdf:resource="http://www.w3.org/2001/XMLSchema#string"/>
  </owl:DatatypeProperty>
  <owl:DatatypeProperty rdf:about="http://example.org/onto/prop/google_container_node_pool_max_surge">
    <rdfs:label>max_surge</rdfs:label>
    <rdfs:comment>The number of additional nodes that can be added to the node pool during an upgrade. Increasing max_surge raises the number of nodes that can be upgraded simultaneously. Can be set to 0 or greater.</rdfs:comment>
    <rdfs:domain rdf:resource="http://example.org/onto/class/google_container_node_pool"/>
    <rdfs:range rdf:resource="http://www.w3.org/2001/XMLSchema#string"/>
  </owl:DatatypeProperty>
  <owl:DatatypeProperty rdf:about="http://example.org/onto/prop/google_container_node_pool_max_unavailable">
    <rdfs:label>max_unavailable</rdfs:label>
    <rdfs:comment>The number of nodes that can be simultaneously unavailable during an upgrade. Increasing max_unavailable raises the number of nodes that can be upgraded in parallel. Can be set to 0 or greater.</rdfs:comment>
    <rdfs:domain rdf:resource="http://example.org/onto/class/google_container_node_pool"/>
    <rdfs:range rdf:resource="http://www.w3.org/2001/XMLSchema#string"/>
  </owl:DatatypeProperty>
  <owl:DatatypeProperty rdf:about="http://example.org/onto/prop/google_container_node_pool_strategy">
    <rdfs:label>strategy</rdfs:label>
    <rdfs:comment>Update strategy for the given nodepool.</rdfs:comment>
    <rdfs:domain rdf:resource="http://example.org/onto/class/google_container_node_pool"/>
    <rdfs:range rdf:resource="http://www.w3.org/2001/XMLSchema#string"/>
  </owl:DatatypeProperty>
  <owl:DatatypeProperty rdf:about="http://example.org/onto/prop/google_container_node_pool_node_pool_soak_duration">
    <rdfs:label>node_pool_soak_duration</rdfs:label>
    <rdfs:comment>Time needed after draining entire blue pool. After this period, blue pool will be cleaned up.</rdfs:comment>
    <rdfs:domain rdf:resource="http://example.org/onto/class/google_container_node_pool"/>
    <rdfs:range rdf:resource="http://www.w3.org/2001/XMLSchema#string"/>
  </owl:DatatypeProperty>
  <owl:DatatypeProperty rdf:about="http://example.org/onto/prop/google_container_node_pool_batch_node_count">
    <rdfs:label>batch_node_count</rdfs:label>
    <rdfs:comment>Number of blue nodes to drain in a batch.</rdfs:comment>
    <rdfs:domain rdf:resource="http://example.org/onto/class/google_container_node_pool"/>
    <rdfs:range rdf:resource="http://www.w3.org/2001/XMLSchema#string"/>
  </owl:DatatypeProperty>
  <owl:DatatypeProperty rdf:about="http://example.org/onto/prop/google_container_node_pool_batch_percentage">
    <rdfs:label>batch_percentage</rdfs:label>
    <rdfs:comment>Percentage of the blue pool nodes to drain in a batch.</rdfs:comment>
    <rdfs:domain rdf:resource="http://example.org/onto/class/google_container_node_pool"/>
    <rdfs:range rdf:resource="http://www.w3.org/2001/XMLSchema#string"/>
  </owl:DatatypeProperty>
  <owl:DatatypeProperty rdf:about="http://example.org/onto/prop/google_container_node_pool_batch_soak_duration">
    <rdfs:label>batch_soak_duration</rdfs:label>
    <rdfs:comment>Soak time after each batch gets drained.</rdfs:comment>
    <rdfs:domain rdf:resource="http://example.org/onto/class/google_container_node_pool"/>
    <rdfs:range rdf:resource="http://www.w3.org/2001/XMLSchema#string"/>
  </owl:DatatypeProperty>
</rdf:RDF>
