<?xml version="1.0" encoding="UTF-8"?>
<rdf:RDF
  xmlns:rdf="http://www.w3.org/1999/02/22-rdf-syntax-ns#"
  xmlns:rdfs="http://www.w3.org/2000/01/rdf-schema#"
  xmlns:owl="http://www.w3.org/2002/07/owl#"
  xmlns:xsd="http://www.w3.org/2001/XMLSchema#"
  xml:base="http://example.org/onto/">
  <owl:Class rdf:about="http://example.org/onto/class/google_dns_managed_zone">
    <rdfs:label>google_dns_managed_zone</rdfs:label>
    <rdfs:comment>#
#     ***     AUTO GENERATED CODE    ***    Type: MMv1     ***
#
# ----------------------------------------------------------------------------
#
#     This code is generated by Magic Modules using the following:
#
#     Configuration: https:#github.com/GoogleCloudPlatform/magic-modules/tree/main/mmv1/products/dns/ManagedZone.yaml
#     Template:      https:#github.com/GoogleCloudPlatform/magic-modules/tree/main/mmv1/templates/terraform/resource.html.markdown.tmpl
#
#     DO NOT EDIT this file directly. Any changes made to this file will be
#     overwritten during the next generation cycle.
#
# ----------------------------------------------------------------------------
subcategory: "Cloud DNS"
description: |-
  A zone is a subtree of the DNS namespace under one administrative
  responsibility.
---</rdfs:comment>
  </owl:Class>
  <owl:DatatypeProperty rdf:about="http://example.org/onto/prop/google_dns_managed_zone_creation_time">
    <rdfs:label>creation_time</rdfs:label>
    <rdfs:comment>The time that this resource was created on the server.
This is in RFC3339 text format.</rdfs:comment>
    <rdfs:domain rdf:resource="http://example.org/onto/class/google_dns_managed_zone"/>
    <rdfs:range rdf:resource="http://www.w3.org/2001/XMLSchema#string"/>
  </owl:DatatypeProperty>
  <owl:DatatypeProperty rdf:about="http://example.org/onto/prop/google_dns_managed_zone_description">
    <rdfs:label>description</rdfs:label>
    <rdfs:comment>A textual description field. Defaults to 'Managed by Terraform'.</rdfs:comment>
    <rdfs:domain rdf:resource="http://example.org/onto/class/google_dns_managed_zone"/>
    <rdfs:range rdf:resource="http://www.w3.org/2001/XMLSchema#string"/>
  </owl:DatatypeProperty>
  <owl:DatatypeProperty rdf:about="http://example.org/onto/prop/google_dns_managed_zone_dns_name">
    <rdfs:label>dns_name</rdfs:label>
    <rdfs:comment>The DNS name of this managed zone, for instance "example.com.".</rdfs:comment>
    <rdfs:domain rdf:resource="http://example.org/onto/class/google_dns_managed_zone"/>
    <rdfs:range rdf:resource="http://www.w3.org/2001/XMLSchema#string"/>
  </owl:DatatypeProperty>
  <owl:DatatypeProperty rdf:about="http://example.org/onto/prop/google_dns_managed_zone_effective_labels">
    <rdfs:label>effective_labels</rdfs:label>
    <rdfs:comment>All of labels (key/value pairs) present on the resource in GCP, including the labels configured through Terraform, other clients and services.</rdfs:comment>
    <rdfs:domain rdf:resource="http://example.org/onto/class/google_dns_managed_zone"/>
    <rdfs:range rdf:resource="http://www.w3.org/2001/XMLSchema#string"/>
  </owl:DatatypeProperty>
  <owl:DatatypeProperty rdf:about="http://example.org/onto/prop/google_dns_managed_zone_force_destroy">
    <rdfs:label>force_destroy</rdfs:label>
    <rdfs:comment>Set this true to delete all records in the zone.</rdfs:comment>
    <rdfs:domain rdf:resource="http://example.org/onto/class/google_dns_managed_zone"/>
    <rdfs:range rdf:resource="http://www.w3.org/2001/XMLSchema#string"/>
  </owl:DatatypeProperty>
  <owl:DatatypeProperty rdf:about="http://example.org/onto/prop/google_dns_managed_zone_id">
    <rdfs:label>id</rdfs:label>
    <rdfs:domain rdf:resource="http://example.org/onto/class/google_dns_managed_zone"/>
    <rdfs:range rdf:resource="http://www.w3.org/2001/XMLSchema#string"/>
  </owl:DatatypeProperty>
  <owl:DatatypeProperty rdf:about="http://example.org/onto/prop/google_dns_managed_zone_labels">
    <rdfs:label>labels</rdfs:label>
    <rdfs:comment>A set of key/value label pairs to assign to this ManagedZone.


**Note**: This field is non-authoritative, and will only manage the labels present in your configuration.
Please refer to the field 'effective_labels' for all of the labels present on the resource.</rdfs:comment>
    <rdfs:domain rdf:resource="http://example.org/onto/class/google_dns_managed_zone"/>
    <rdfs:range rdf:resource="http://www.w3.org/2001/XMLSchema#string"/>
  </owl:DatatypeProperty>
  <owl:DatatypeProperty rdf:about="http://example.org/onto/prop/google_dns_managed_zone_managed_zone_id">
    <rdfs:label>managed_zone_id</rdfs:label>
    <rdfs:comment>Unique identifier for the resource; defined by the server.</rdfs:comment>
    <rdfs:domain rdf:resource="http://example.org/onto/class/google_dns_managed_zone"/>
    <rdfs:range rdf:resource="http://www.w3.org/2001/XMLSchema#string"/>
  </owl:DatatypeProperty>
  <owl:DatatypeProperty rdf:about="http://example.org/onto/prop/google_dns_managed_zone_name">
    <rdfs:label>name</rdfs:label>
    <rdfs:comment>User assigned name for this resource.
Must be unique within the project.</rdfs:comment>
    <rdfs:domain rdf:resource="http://example.org/onto/class/google_dns_managed_zone"/>
    <rdfs:range rdf:resource="http://www.w3.org/2001/XMLSchema#string"/>
  </owl:DatatypeProperty>
  <owl:DatatypeProperty rdf:about="http://example.org/onto/prop/google_dns_managed_zone_name_servers">
    <rdfs:label>name_servers</rdfs:label>
    <rdfs:comment>Delegate your managed_zone to these virtual name servers;
defined by the server</rdfs:comment>
    <rdfs:domain rdf:resource="http://example.org/onto/class/google_dns_managed_zone"/>
    <rdfs:range rdf:resource="http://www.w3.org/2001/XMLSchema#string"/>
  </owl:DatatypeProperty>
  <owl:DatatypeProperty rdf:about="http://example.org/onto/prop/google_dns_managed_zone_project">
    <rdfs:label>project</rdfs:label>
    <rdfs:domain rdf:resource="http://example.org/onto/class/google_dns_managed_zone"/>
    <rdfs:range rdf:resource="http://www.w3.org/2001/XMLSchema#string"/>
  </owl:DatatypeProperty>
  <owl:DatatypeProperty rdf:about="http://example.org/onto/prop/google_dns_managed_zone_terraform_labels">
    <rdfs:label>terraform_labels</rdfs:label>
    <rdfs:comment>The combination of labels configured directly on the resource
 and default labels configured on the provider.</rdfs:comment>
    <rdfs:domain rdf:resource="http://example.org/onto/class/google_dns_managed_zone"/>
    <rdfs:range rdf:resource="http://www.w3.org/2001/XMLSchema#string"/>
  </owl:DatatypeProperty>
  <owl:DatatypeProperty rdf:about="http://example.org/onto/prop/google_dns_managed_zone_visibility">
    <rdfs:label>visibility</rdfs:label>
    <rdfs:comment>The zone's visibility: public zones are exposed to the Internet,
while private zones are visible only to Virtual Private Cloud resources. Default value: "public" Possible values: ["private", "public"]</rdfs:comment>
    <rdfs:domain rdf:resource="http://example.org/onto/class/google_dns_managed_zone"/>
    <rdfs:range rdf:resource="http://www.w3.org/2001/XMLSchema#string"/>
  </owl:DatatypeProperty>
  <owl:DatatypeProperty rdf:about="http://example.org/onto/prop/google_dns_managed_zone_enable_logging">
    <rdfs:label>enable_logging</rdfs:label>
    <rdfs:comment>If set, enable query logging for this ManagedZone. False by default, making logging opt-in.</rdfs:comment>
    <rdfs:domain rdf:resource="http://example.org/onto/class/google_dns_managed_zone"/>
    <rdfs:range rdf:resource="http://www.w3.org/2001/XMLSchema#string"/>
  </owl:DatatypeProperty>
  <owl:DatatypeProperty rdf:about="http://example.org/onto/prop/google_dns_managed_zone_kind">
    <rdfs:label>kind</rdfs:label>
    <rdfs:comment>Identifies what kind of resource this is</rdfs:comment>
    <rdfs:domain rdf:resource="http://example.org/onto/class/google_dns_managed_zone"/>
    <rdfs:range rdf:resource="http://www.w3.org/2001/XMLSchema#string"/>
  </owl:DatatypeProperty>
  <owl:DatatypeProperty rdf:about="http://example.org/onto/prop/google_dns_managed_zone_non_existence">
    <rdfs:label>non_existence</rdfs:label>
    <rdfs:comment>Specifies the mechanism used to provide authenticated denial-of-existence responses.
non_existence can only be updated when the state is 'off'. Possible values: ["nsec", "nsec3"]</rdfs:comment>
    <rdfs:domain rdf:resource="http://example.org/onto/class/google_dns_managed_zone"/>
    <rdfs:range rdf:resource="http://www.w3.org/2001/XMLSchema#string"/>
  </owl:DatatypeProperty>
  <owl:DatatypeProperty rdf:about="http://example.org/onto/prop/google_dns_managed_zone_state">
    <rdfs:label>state</rdfs:label>
    <rdfs:comment>Specifies whether DNSSEC is enabled, and what mode it is in Possible values: ["off", "on", "transfer"]</rdfs:comment>
    <rdfs:domain rdf:resource="http://example.org/onto/class/google_dns_managed_zone"/>
    <rdfs:range rdf:resource="http://www.w3.org/2001/XMLSchema#string"/>
  </owl:DatatypeProperty>
  <owl:DatatypeProperty rdf:about="http://example.org/onto/prop/google_dns_managed_zone_algorithm">
    <rdfs:label>algorithm</rdfs:label>
    <rdfs:comment>String mnemonic specifying the DNSSEC algorithm of this key Possible values: ["ecdsap256sha256", "ecdsap384sha384", "rsasha1", "rsasha256", "rsasha512"]</rdfs:comment>
    <rdfs:domain rdf:resource="http://example.org/onto/class/google_dns_managed_zone"/>
    <rdfs:range rdf:resource="http://www.w3.org/2001/XMLSchema#string"/>
  </owl:DatatypeProperty>
  <owl:DatatypeProperty rdf:about="http://example.org/onto/prop/google_dns_managed_zone_key_length">
    <rdfs:label>key_length</rdfs:label>
    <rdfs:comment>Length of the keys in bits</rdfs:comment>
    <rdfs:domain rdf:resource="http://example.org/onto/class/google_dns_managed_zone"/>
    <rdfs:range rdf:resource="http://www.w3.org/2001/XMLSchema#string"/>
  </owl:DatatypeProperty>
  <owl:DatatypeProperty rdf:about="http://example.org/onto/prop/google_dns_managed_zone_key_type">
    <rdfs:label>key_type</rdfs:label>
    <rdfs:comment>Specifies whether this is a key signing key (KSK) or a zone
signing key (ZSK). Key signing keys have the Secure Entry
Point flag set and, when active, will only be used to sign
resource record sets of type DNSKEY. Zone signing keys do
not have the Secure Entry Point flag set and will be used
to sign all other types of resource record sets. Possible values: ["keySigning", "zoneSigning"]</rdfs:comment>
    <rdfs:domain rdf:resource="http://example.org/onto/class/google_dns_managed_zone"/>
    <rdfs:range rdf:resource="http://www.w3.org/2001/XMLSchema#string"/>
  </owl:DatatypeProperty>
  <owl:DatatypeProperty rdf:about="http://example.org/onto/prop/google_dns_managed_zone_kind">
    <rdfs:label>kind</rdfs:label>
    <rdfs:comment>Identifies what kind of resource this is</rdfs:comment>
    <rdfs:domain rdf:resource="http://example.org/onto/class/google_dns_managed_zone"/>
    <rdfs:range rdf:resource="http://www.w3.org/2001/XMLSchema#string"/>
  </owl:DatatypeProperty>
  <owl:DatatypeProperty rdf:about="http://example.org/onto/prop/google_dns_managed_zone_domain_name">
    <rdfs:label>domain_name</rdfs:label>
    <rdfs:comment>Fully qualified domain name for the forwarding target.</rdfs:comment>
    <rdfs:domain rdf:resource="http://example.org/onto/class/google_dns_managed_zone"/>
    <rdfs:range rdf:resource="http://www.w3.org/2001/XMLSchema#string"/>
  </owl:DatatypeProperty>
  <owl:DatatypeProperty rdf:about="http://example.org/onto/prop/google_dns_managed_zone_forwarding_path">
    <rdfs:label>forwarding_path</rdfs:label>
    <rdfs:comment>Forwarding path for this TargetNameServer. If unset or 'default' Cloud DNS will make forwarding
decision based on address ranges, i.e. RFC1918 addresses go to the VPC, Non-RFC1918 addresses go
to the Internet. When set to 'private', Cloud DNS will always send queries through VPC for this target Possible values: ["default", "private"]</rdfs:comment>
    <rdfs:domain rdf:resource="http://example.org/onto/class/google_dns_managed_zone"/>
    <rdfs:range rdf:resource="http://www.w3.org/2001/XMLSchema#string"/>
  </owl:DatatypeProperty>
  <owl:DatatypeProperty rdf:about="http://example.org/onto/prop/google_dns_managed_zone_ipv4_address">
    <rdfs:label>ipv4_address</rdfs:label>
    <rdfs:comment>IPv4 address of a target name server.</rdfs:comment>
    <rdfs:domain rdf:resource="http://example.org/onto/class/google_dns_managed_zone"/>
    <rdfs:range rdf:resource="http://www.w3.org/2001/XMLSchema#string"/>
  </owl:DatatypeProperty>
  <owl:DatatypeProperty rdf:about="http://example.org/onto/prop/google_dns_managed_zone_network_url">
    <rdfs:label>network_url</rdfs:label>
    <rdfs:comment>The id or fully qualified URL of the VPC network to forward queries to.
This should be formatted like 'projects/{project}/global/networks/{network}' or
'https://www.googleapis.com/compute/v1/projects/{project}/global/networks/{network}'</rdfs:comment>
    <rdfs:domain rdf:resource="http://example.org/onto/class/google_dns_managed_zone"/>
    <rdfs:range rdf:resource="http://www.w3.org/2001/XMLSchema#string"/>
  </owl:DatatypeProperty>
  <owl:DatatypeProperty rdf:about="http://example.org/onto/prop/google_dns_managed_zone_gke_cluster_name">
    <rdfs:label>gke_cluster_name</rdfs:label>
    <rdfs:comment>The resource name of the cluster to bind this ManagedZone to.
This should be specified in the format like
'projects/*/locations/*/clusters/*'</rdfs:comment>
    <rdfs:domain rdf:resource="http://example.org/onto/class/google_dns_managed_zone"/>
    <rdfs:range rdf:resource="http://www.w3.org/2001/XMLSchema#string"/>
  </owl:DatatypeProperty>
  <owl:DatatypeProperty rdf:about="http://example.org/onto/prop/google_dns_managed_zone_network_url">
    <rdfs:label>network_url</rdfs:label>
    <rdfs:comment>The id or fully qualified URL of the VPC network to bind to.
This should be formatted like 'projects/{project}/global/networks/{network}' or
'https://www.googleapis.com/compute/v1/projects/{project}/global/networks/{network}'</rdfs:comment>
    <rdfs:domain rdf:resource="http://example.org/onto/class/google_dns_managed_zone"/>
    <rdfs:range rdf:resource="http://www.w3.org/2001/XMLSchema#string"/>
  </owl:DatatypeProperty>
  <owl:DatatypeProperty rdf:about="http://example.org/onto/prop/google_dns_managed_zone_create">
    <rdfs:label>create</rdfs:label>
    <rdfs:domain rdf:resource="http://example.org/onto/class/google_dns_managed_zone"/>
    <rdfs:range rdf:resource="http://www.w3.org/2001/XMLSchema#string"/>
  </owl:DatatypeProperty>
  <owl:DatatypeProperty rdf:about="http://example.org/onto/prop/google_dns_managed_zone_delete">
    <rdfs:label>delete</rdfs:label>
    <rdfs:domain rdf:resource="http://example.org/onto/class/google_dns_managed_zone"/>
    <rdfs:range rdf:resource="http://www.w3.org/2001/XMLSchema#string"/>
  </owl:DatatypeProperty>
  <owl:DatatypeProperty rdf:about="http://example.org/onto/prop/google_dns_managed_zone_update">
    <rdfs:label>update</rdfs:label>
    <rdfs:domain rdf:resource="http://example.org/onto/class/google_dns_managed_zone"/>
    <rdfs:range rdf:resource="http://www.w3.org/2001/XMLSchema#string"/>
  </owl:DatatypeProperty>
</rdf:RDF>
