<?xml version="1.0" encoding="UTF-8"?>
<rdf:RDF
  xmlns:rdf="http://www.w3.org/1999/02/22-rdf-syntax-ns#"
  xmlns:rdfs="http://www.w3.org/2000/01/rdf-schema#"
  xmlns:owl="http://www.w3.org/2002/07/owl#"
  xmlns:xsd="http://www.w3.org/2001/XMLSchema#"
  xml:base="http://example.org/onto/">
  <owl:Class rdf:about="http://example.org/onto/class/google_apigee_security_action">
    <rdfs:label>google_apigee_security_action</rdfs:label>
    <rdfs:comment>#
#     ***     AUTO GENERATED CODE    ***    Type: MMv1     ***
#
# ----------------------------------------------------------------------------
#
#     This code is generated by Magic Modules using the following:
#
#     Configuration: https:#github.com/GoogleCloudPlatform/magic-modules/tree/main/mmv1/products/apigee/SecurityAction.yaml
#     Template:      https:#github.com/GoogleCloudPlatform/magic-modules/tree/main/mmv1/templates/terraform/resource.html.markdown.tmpl
#
#     DO NOT EDIT this file directly. Any changes made to this file will be
#     overwritten during the next generation cycle.
#
# ----------------------------------------------------------------------------
subcategory: "Apigee"
description: |-
  A SecurityAction is rule that can be enforced at an environment level.
---</rdfs:comment>
  </owl:Class>
  <owl:DatatypeProperty rdf:about="http://example.org/onto/prop/google_apigee_security_action_api_proxies">
    <rdfs:label>api_proxies</rdfs:label>
    <rdfs:comment>If unset, this would apply to all proxies in the environment.
If set, this action is enforced only if at least one proxy in the repeated
list is deployed at the time of enforcement. If set, several restrictions are enforced on SecurityActions.
There can be at most 100 enabled actions with proxies set in an env.
Several other restrictions apply on conditions and are detailed later.</rdfs:comment>
    <rdfs:domain rdf:resource="http://example.org/onto/class/google_apigee_security_action"/>
    <rdfs:range rdf:resource="http://www.w3.org/2001/XMLSchema#string"/>
  </owl:DatatypeProperty>
  <owl:DatatypeProperty rdf:about="http://example.org/onto/prop/google_apigee_security_action_create_time">
    <rdfs:label>create_time</rdfs:label>
    <rdfs:comment>The create time for this SecurityAction.
Uses RFC 3339, where generated output will always be Z-normalized and uses 0, 3, 6 or 9 fractional digits.
Offsets other than "Z" are also accepted. Examples: "2014-10-02T15:01:23Z", "2014-10-02T15:01:23.045123456Z" or "2014-10-02T15:01:23+05:30".</rdfs:comment>
    <rdfs:domain rdf:resource="http://example.org/onto/class/google_apigee_security_action"/>
    <rdfs:range rdf:resource="http://www.w3.org/2001/XMLSchema#string"/>
  </owl:DatatypeProperty>
  <owl:DatatypeProperty rdf:about="http://example.org/onto/prop/google_apigee_security_action_description">
    <rdfs:label>description</rdfs:label>
    <rdfs:comment>An optional user provided description of the SecurityAction.</rdfs:comment>
    <rdfs:domain rdf:resource="http://example.org/onto/class/google_apigee_security_action"/>
    <rdfs:range rdf:resource="http://www.w3.org/2001/XMLSchema#string"/>
  </owl:DatatypeProperty>
  <owl:DatatypeProperty rdf:about="http://example.org/onto/prop/google_apigee_security_action_env_id">
    <rdfs:label>env_id</rdfs:label>
    <rdfs:comment>The Apigee environment that this security action applies to.</rdfs:comment>
    <rdfs:domain rdf:resource="http://example.org/onto/class/google_apigee_security_action"/>
    <rdfs:range rdf:resource="http://www.w3.org/2001/XMLSchema#string"/>
  </owl:DatatypeProperty>
  <owl:DatatypeProperty rdf:about="http://example.org/onto/prop/google_apigee_security_action_expire_time">
    <rdfs:label>expire_time</rdfs:label>
    <rdfs:comment>The expiration for this SecurityAction.
Uses RFC 3339, where generated output will always be Z-normalized and uses 0, 3, 6 or 9
fractional digits. Offsets other than "Z" are also accepted.
Examples: "2014-10-02T15:01:23Z", "2014-10-02T15:01:23.045123456Z" or "2014-10-02T15:01:23+05:30".</rdfs:comment>
    <rdfs:domain rdf:resource="http://example.org/onto/class/google_apigee_security_action"/>
    <rdfs:range rdf:resource="http://www.w3.org/2001/XMLSchema#string"/>
  </owl:DatatypeProperty>
  <owl:DatatypeProperty rdf:about="http://example.org/onto/prop/google_apigee_security_action_id">
    <rdfs:label>id</rdfs:label>
    <rdfs:domain rdf:resource="http://example.org/onto/class/google_apigee_security_action"/>
    <rdfs:range rdf:resource="http://www.w3.org/2001/XMLSchema#string"/>
  </owl:DatatypeProperty>
  <owl:DatatypeProperty rdf:about="http://example.org/onto/prop/google_apigee_security_action_org_id">
    <rdfs:label>org_id</rdfs:label>
    <rdfs:comment>The organization that this security action applies to.</rdfs:comment>
    <rdfs:domain rdf:resource="http://example.org/onto/class/google_apigee_security_action"/>
    <rdfs:range rdf:resource="http://www.w3.org/2001/XMLSchema#string"/>
  </owl:DatatypeProperty>
  <owl:DatatypeProperty rdf:about="http://example.org/onto/prop/google_apigee_security_action_security_action_id">
    <rdfs:label>security_action_id</rdfs:label>
    <rdfs:comment>The ID to use for the SecurityAction, which will become the final component of the action's resource name.
This value should be 0-61 characters, and valid format is (^a-z?$).</rdfs:comment>
    <rdfs:domain rdf:resource="http://example.org/onto/class/google_apigee_security_action"/>
    <rdfs:range rdf:resource="http://www.w3.org/2001/XMLSchema#string"/>
  </owl:DatatypeProperty>
  <owl:DatatypeProperty rdf:about="http://example.org/onto/prop/google_apigee_security_action_state">
    <rdfs:label>state</rdfs:label>
    <rdfs:comment>Only an ENABLED SecurityAction is enforced. An ENABLED SecurityAction past its expiration time will not be enforced. Possible values: ["ENABLED", "DISABLED"]</rdfs:comment>
    <rdfs:domain rdf:resource="http://example.org/onto/class/google_apigee_security_action"/>
    <rdfs:range rdf:resource="http://www.w3.org/2001/XMLSchema#string"/>
  </owl:DatatypeProperty>
  <owl:DatatypeProperty rdf:about="http://example.org/onto/prop/google_apigee_security_action_ttl">
    <rdfs:label>ttl</rdfs:label>
    <rdfs:comment>The TTL for this SecurityAction.
A duration in seconds with up to nine fractional digits, ending with 's'. Example: "3.5s".</rdfs:comment>
    <rdfs:domain rdf:resource="http://example.org/onto/class/google_apigee_security_action"/>
    <rdfs:range rdf:resource="http://www.w3.org/2001/XMLSchema#string"/>
  </owl:DatatypeProperty>
  <owl:DatatypeProperty rdf:about="http://example.org/onto/prop/google_apigee_security_action_update_time">
    <rdfs:label>update_time</rdfs:label>
    <rdfs:comment>The update time for this SecurityAction. This reflects when this SecurityAction changed states.
Uses RFC 3339, where generated output will always be Z-normalized and uses 0, 3, 6 or 9 fractional digits.
Offsets other than "Z" are also accepted. Examples: "2014-10-02T15:01:23Z", "2014-10-02T15:01:23.045123456Z" or "2014-10-02T15:01:23+05:30".</rdfs:comment>
    <rdfs:domain rdf:resource="http://example.org/onto/class/google_apigee_security_action"/>
    <rdfs:range rdf:resource="http://www.w3.org/2001/XMLSchema#string"/>
  </owl:DatatypeProperty>
  <owl:DatatypeProperty rdf:about="http://example.org/onto/prop/google_apigee_security_action_access_tokens">
    <rdfs:label>access_tokens</rdfs:label>
    <rdfs:comment>A list of accessTokens. Limit 1000 per action.</rdfs:comment>
    <rdfs:domain rdf:resource="http://example.org/onto/class/google_apigee_security_action"/>
    <rdfs:range rdf:resource="http://www.w3.org/2001/XMLSchema#string"/>
  </owl:DatatypeProperty>
  <owl:DatatypeProperty rdf:about="http://example.org/onto/prop/google_apigee_security_action_api_keys">
    <rdfs:label>api_keys</rdfs:label>
    <rdfs:comment>A list of API keys. Limit 1000 per action.</rdfs:comment>
    <rdfs:domain rdf:resource="http://example.org/onto/class/google_apigee_security_action"/>
    <rdfs:range rdf:resource="http://www.w3.org/2001/XMLSchema#string"/>
  </owl:DatatypeProperty>
  <owl:DatatypeProperty rdf:about="http://example.org/onto/prop/google_apigee_security_action_api_products">
    <rdfs:label>api_products</rdfs:label>
    <rdfs:comment>A list of API Products. Limit 1000 per action.</rdfs:comment>
    <rdfs:domain rdf:resource="http://example.org/onto/class/google_apigee_security_action"/>
    <rdfs:range rdf:resource="http://www.w3.org/2001/XMLSchema#string"/>
  </owl:DatatypeProperty>
  <owl:DatatypeProperty rdf:about="http://example.org/onto/prop/google_apigee_security_action_asns">
    <rdfs:label>asns</rdfs:label>
    <rdfs:comment>A list of ASN numbers to act on, e.g. 23. https://en.wikipedia.org/wiki/Autonomous_system_(Internet)
This uses int64 instead of uint32 because of https://linter.aip.dev/141/forbidden-types.</rdfs:comment>
    <rdfs:domain rdf:resource="http://example.org/onto/class/google_apigee_security_action"/>
    <rdfs:range rdf:resource="http://www.w3.org/2001/XMLSchema#string"/>
  </owl:DatatypeProperty>
  <owl:DatatypeProperty rdf:about="http://example.org/onto/prop/google_apigee_security_action_bot_reasons">
    <rdfs:label>bot_reasons</rdfs:label>
    <rdfs:comment>A list of Bot Reasons. Current options: Flooder, Brute Guessor, Static Content Scraper,
OAuth Abuser, Robot Abuser, TorListRule, Advanced Anomaly Detection, Advanced API Scraper,
Search Engine Crawlers, Public Clouds, Public Cloud AWS, Public Cloud Azure, and Public Cloud Google.</rdfs:comment>
    <rdfs:domain rdf:resource="http://example.org/onto/class/google_apigee_security_action"/>
    <rdfs:range rdf:resource="http://www.w3.org/2001/XMLSchema#string"/>
  </owl:DatatypeProperty>
  <owl:DatatypeProperty rdf:about="http://example.org/onto/prop/google_apigee_security_action_developer_apps">
    <rdfs:label>developer_apps</rdfs:label>
    <rdfs:comment>A list of developer apps. Limit 1000 per action.</rdfs:comment>
    <rdfs:domain rdf:resource="http://example.org/onto/class/google_apigee_security_action"/>
    <rdfs:range rdf:resource="http://www.w3.org/2001/XMLSchema#string"/>
  </owl:DatatypeProperty>
  <owl:DatatypeProperty rdf:about="http://example.org/onto/prop/google_apigee_security_action_developers">
    <rdfs:label>developers</rdfs:label>
    <rdfs:comment>A list of developers. Limit 1000 per action.</rdfs:comment>
    <rdfs:domain rdf:resource="http://example.org/onto/class/google_apigee_security_action"/>
    <rdfs:range rdf:resource="http://www.w3.org/2001/XMLSchema#string"/>
  </owl:DatatypeProperty>
  <owl:DatatypeProperty rdf:about="http://example.org/onto/prop/google_apigee_security_action_http_methods">
    <rdfs:label>http_methods</rdfs:label>
    <rdfs:comment>Act only on particular HTTP methods. E.g. A read-only API can block POST/PUT/DELETE methods.
Accepted values are: GET, HEAD, POST, PUT, DELETE, CONNECT, OPTIONS, TRACE and PATCH.</rdfs:comment>
    <rdfs:domain rdf:resource="http://example.org/onto/class/google_apigee_security_action"/>
    <rdfs:range rdf:resource="http://www.w3.org/2001/XMLSchema#string"/>
  </owl:DatatypeProperty>
  <owl:DatatypeProperty rdf:about="http://example.org/onto/prop/google_apigee_security_action_ip_address_ranges">
    <rdfs:label>ip_address_ranges</rdfs:label>
    <rdfs:comment>A list of IP addresses. This could be either IPv4 or IPv6. Limited to 100 per action.</rdfs:comment>
    <rdfs:domain rdf:resource="http://example.org/onto/class/google_apigee_security_action"/>
    <rdfs:range rdf:resource="http://www.w3.org/2001/XMLSchema#string"/>
  </owl:DatatypeProperty>
  <owl:DatatypeProperty rdf:about="http://example.org/onto/prop/google_apigee_security_action_region_codes">
    <rdfs:label>region_codes</rdfs:label>
    <rdfs:comment>A list of countries/region codes to act on, e.g. US. This follows https://en.wikipedia.org/wiki/ISO_3166-1_alpha-2.</rdfs:comment>
    <rdfs:domain rdf:resource="http://example.org/onto/class/google_apigee_security_action"/>
    <rdfs:range rdf:resource="http://www.w3.org/2001/XMLSchema#string"/>
  </owl:DatatypeProperty>
  <owl:DatatypeProperty rdf:about="http://example.org/onto/prop/google_apigee_security_action_user_agents">
    <rdfs:label>user_agents</rdfs:label>
    <rdfs:comment>A list of user agents to deny. We look for exact matches. Limit 50 per action.</rdfs:comment>
    <rdfs:domain rdf:resource="http://example.org/onto/class/google_apigee_security_action"/>
    <rdfs:range rdf:resource="http://www.w3.org/2001/XMLSchema#string"/>
  </owl:DatatypeProperty>
  <owl:DatatypeProperty rdf:about="http://example.org/onto/prop/google_apigee_security_action_response_code">
    <rdfs:label>response_code</rdfs:label>
    <rdfs:comment>The HTTP response code if the Action = DENY.</rdfs:comment>
    <rdfs:domain rdf:resource="http://example.org/onto/class/google_apigee_security_action"/>
    <rdfs:range rdf:resource="http://www.w3.org/2001/XMLSchema#string"/>
  </owl:DatatypeProperty>
  <owl:DatatypeProperty rdf:about="http://example.org/onto/prop/google_apigee_security_action_name">
    <rdfs:label>name</rdfs:label>
    <rdfs:comment>The header name to be sent to the target.</rdfs:comment>
    <rdfs:domain rdf:resource="http://example.org/onto/class/google_apigee_security_action"/>
    <rdfs:range rdf:resource="http://www.w3.org/2001/XMLSchema#string"/>
  </owl:DatatypeProperty>
  <owl:DatatypeProperty rdf:about="http://example.org/onto/prop/google_apigee_security_action_value">
    <rdfs:label>value</rdfs:label>
    <rdfs:comment>The header value to be sent to the target.</rdfs:comment>
    <rdfs:domain rdf:resource="http://example.org/onto/class/google_apigee_security_action"/>
    <rdfs:range rdf:resource="http://www.w3.org/2001/XMLSchema#string"/>
  </owl:DatatypeProperty>
  <owl:DatatypeProperty rdf:about="http://example.org/onto/prop/google_apigee_security_action_create">
    <rdfs:label>create</rdfs:label>
    <rdfs:domain rdf:resource="http://example.org/onto/class/google_apigee_security_action"/>
    <rdfs:range rdf:resource="http://www.w3.org/2001/XMLSchema#string"/>
  </owl:DatatypeProperty>
  <owl:DatatypeProperty rdf:about="http://example.org/onto/prop/google_apigee_security_action_delete">
    <rdfs:label>delete</rdfs:label>
    <rdfs:domain rdf:resource="http://example.org/onto/class/google_apigee_security_action"/>
    <rdfs:range rdf:resource="http://www.w3.org/2001/XMLSchema#string"/>
  </owl:DatatypeProperty>
</rdf:RDF>
