<?xml version="1.0" encoding="UTF-8"?>
<rdf:RDF
  xmlns:rdf="http://www.w3.org/1999/02/22-rdf-syntax-ns#"
  xmlns:rdfs="http://www.w3.org/2000/01/rdf-schema#"
  xmlns:owl="http://www.w3.org/2002/07/owl#"
  xmlns:xsd="http://www.w3.org/2001/XMLSchema#"
  xml:base="http://example.org/onto/">
  <owl:Class rdf:about="http://example.org/onto/class/google_app_engine_standard_app_version">
    <rdfs:label>google_app_engine_standard_app_version</rdfs:label>
    <rdfs:comment>#
#     ***     AUTO GENERATED CODE    ***    Type: MMv1     ***
#
# ----------------------------------------------------------------------------
#
#     This code is generated by Magic Modules using the following:
#
#     Configuration: https:#github.com/GoogleCloudPlatform/magic-modules/tree/main/mmv1/products/appengine/StandardAppVersion.yaml
#     Template:      https:#github.com/GoogleCloudPlatform/magic-modules/tree/main/mmv1/templates/terraform/resource.html.markdown.tmpl
#
#     DO NOT EDIT this file directly. Any changes made to this file will be
#     overwritten during the next generation cycle.
#
# ----------------------------------------------------------------------------
subcategory: "App Engine"
description: |-
  Standard App Version resource to create a new version of standard GAE Application.
---</rdfs:comment>
  </owl:Class>
  <owl:DatatypeProperty rdf:about="http://example.org/onto/prop/google_app_engine_standard_app_version_app_engine_apis">
    <rdfs:label>app_engine_apis</rdfs:label>
    <rdfs:comment>Allows App Engine second generation runtimes to access the legacy bundled services.</rdfs:comment>
    <rdfs:domain rdf:resource="http://example.org/onto/class/google_app_engine_standard_app_version"/>
    <rdfs:range rdf:resource="http://www.w3.org/2001/XMLSchema#string"/>
  </owl:DatatypeProperty>
  <owl:DatatypeProperty rdf:about="http://example.org/onto/prop/google_app_engine_standard_app_version_delete_service_on_destroy">
    <rdfs:label>delete_service_on_destroy</rdfs:label>
    <rdfs:comment>If set to 'true', the service will be deleted if it is the last version.</rdfs:comment>
    <rdfs:domain rdf:resource="http://example.org/onto/class/google_app_engine_standard_app_version"/>
    <rdfs:range rdf:resource="http://www.w3.org/2001/XMLSchema#string"/>
  </owl:DatatypeProperty>
  <owl:DatatypeProperty rdf:about="http://example.org/onto/prop/google_app_engine_standard_app_version_env_variables">
    <rdfs:label>env_variables</rdfs:label>
    <rdfs:comment>Environment variables available to the application.</rdfs:comment>
    <rdfs:domain rdf:resource="http://example.org/onto/class/google_app_engine_standard_app_version"/>
    <rdfs:range rdf:resource="http://www.w3.org/2001/XMLSchema#string"/>
  </owl:DatatypeProperty>
  <owl:DatatypeProperty rdf:about="http://example.org/onto/prop/google_app_engine_standard_app_version_id">
    <rdfs:label>id</rdfs:label>
    <rdfs:domain rdf:resource="http://example.org/onto/class/google_app_engine_standard_app_version"/>
    <rdfs:range rdf:resource="http://www.w3.org/2001/XMLSchema#string"/>
  </owl:DatatypeProperty>
  <owl:DatatypeProperty rdf:about="http://example.org/onto/prop/google_app_engine_standard_app_version_inbound_services">
    <rdfs:label>inbound_services</rdfs:label>
    <rdfs:comment>A list of the types of messages that this application is able to receive. Possible values: ["INBOUND_SERVICE_MAIL", "INBOUND_SERVICE_MAIL_BOUNCE", "INBOUND_SERVICE_XMPP_ERROR", "INBOUND_SERVICE_XMPP_MESSAGE", "INBOUND_SERVICE_XMPP_SUBSCRIBE", "INBOUND_SERVICE_XMPP_PRESENCE", "INBOUND_SERVICE_CHANNEL_PRESENCE", "INBOUND_SERVICE_WARMUP"]</rdfs:comment>
    <rdfs:domain rdf:resource="http://example.org/onto/class/google_app_engine_standard_app_version"/>
    <rdfs:range rdf:resource="http://www.w3.org/2001/XMLSchema#string"/>
  </owl:DatatypeProperty>
  <owl:DatatypeProperty rdf:about="http://example.org/onto/prop/google_app_engine_standard_app_version_instance_class">
    <rdfs:label>instance_class</rdfs:label>
    <rdfs:comment>Instance class that is used to run this version. Valid values are
AutomaticScaling: F1, F2, F4, F4_1G
BasicScaling or ManualScaling: B1, B2, B4, B4_1G, B8
Defaults to F1 for AutomaticScaling and B2 for ManualScaling and BasicScaling. If no scaling is specified, AutomaticScaling is chosen.</rdfs:comment>
    <rdfs:domain rdf:resource="http://example.org/onto/class/google_app_engine_standard_app_version"/>
    <rdfs:range rdf:resource="http://www.w3.org/2001/XMLSchema#string"/>
  </owl:DatatypeProperty>
  <owl:DatatypeProperty rdf:about="http://example.org/onto/prop/google_app_engine_standard_app_version_name">
    <rdfs:label>name</rdfs:label>
    <rdfs:comment>Full path to the Version resource in the API. Example, "v1".</rdfs:comment>
    <rdfs:domain rdf:resource="http://example.org/onto/class/google_app_engine_standard_app_version"/>
    <rdfs:range rdf:resource="http://www.w3.org/2001/XMLSchema#string"/>
  </owl:DatatypeProperty>
  <owl:DatatypeProperty rdf:about="http://example.org/onto/prop/google_app_engine_standard_app_version_noop_on_destroy">
    <rdfs:label>noop_on_destroy</rdfs:label>
    <rdfs:comment>If set to 'true', the application version will not be deleted.</rdfs:comment>
    <rdfs:domain rdf:resource="http://example.org/onto/class/google_app_engine_standard_app_version"/>
    <rdfs:range rdf:resource="http://www.w3.org/2001/XMLSchema#string"/>
  </owl:DatatypeProperty>
  <owl:DatatypeProperty rdf:about="http://example.org/onto/prop/google_app_engine_standard_app_version_project">
    <rdfs:label>project</rdfs:label>
    <rdfs:domain rdf:resource="http://example.org/onto/class/google_app_engine_standard_app_version"/>
    <rdfs:range rdf:resource="http://www.w3.org/2001/XMLSchema#string"/>
  </owl:DatatypeProperty>
  <owl:DatatypeProperty rdf:about="http://example.org/onto/prop/google_app_engine_standard_app_version_runtime">
    <rdfs:label>runtime</rdfs:label>
    <rdfs:comment>Desired runtime. Example python27.</rdfs:comment>
    <rdfs:domain rdf:resource="http://example.org/onto/class/google_app_engine_standard_app_version"/>
    <rdfs:range rdf:resource="http://www.w3.org/2001/XMLSchema#string"/>
  </owl:DatatypeProperty>
  <owl:DatatypeProperty rdf:about="http://example.org/onto/prop/google_app_engine_standard_app_version_runtime_api_version">
    <rdfs:label>runtime_api_version</rdfs:label>
    <rdfs:comment>The version of the API in the given runtime environment.
Please see the app.yaml reference for valid values at 'https://cloud.google.com/appengine/docs/standard/<language>/config/appref'\
Substitute '<language>' with 'python', 'java', 'php', 'ruby', 'go' or 'nodejs'.</rdfs:comment>
    <rdfs:domain rdf:resource="http://example.org/onto/class/google_app_engine_standard_app_version"/>
    <rdfs:range rdf:resource="http://www.w3.org/2001/XMLSchema#string"/>
  </owl:DatatypeProperty>
  <owl:DatatypeProperty rdf:about="http://example.org/onto/prop/google_app_engine_standard_app_version_service">
    <rdfs:label>service</rdfs:label>
    <rdfs:comment>AppEngine service resource</rdfs:comment>
    <rdfs:domain rdf:resource="http://example.org/onto/class/google_app_engine_standard_app_version"/>
    <rdfs:range rdf:resource="http://www.w3.org/2001/XMLSchema#string"/>
  </owl:DatatypeProperty>
  <owl:DatatypeProperty rdf:about="http://example.org/onto/prop/google_app_engine_standard_app_version_service_account">
    <rdfs:label>service_account</rdfs:label>
    <rdfs:comment>The identity that the deployed version will run as. Admin API will use the App Engine Appspot service account as default if this field is neither provided in app.yaml file nor through CLI flag.</rdfs:comment>
    <rdfs:domain rdf:resource="http://example.org/onto/class/google_app_engine_standard_app_version"/>
    <rdfs:range rdf:resource="http://www.w3.org/2001/XMLSchema#string"/>
  </owl:DatatypeProperty>
  <owl:DatatypeProperty rdf:about="http://example.org/onto/prop/google_app_engine_standard_app_version_threadsafe">
    <rdfs:label>threadsafe</rdfs:label>
    <rdfs:comment>Whether multiple requests can be dispatched to this version at once.</rdfs:comment>
    <rdfs:domain rdf:resource="http://example.org/onto/class/google_app_engine_standard_app_version"/>
    <rdfs:range rdf:resource="http://www.w3.org/2001/XMLSchema#string"/>
  </owl:DatatypeProperty>
  <owl:DatatypeProperty rdf:about="http://example.org/onto/prop/google_app_engine_standard_app_version_version_id">
    <rdfs:label>version_id</rdfs:label>
    <rdfs:comment>Relative name of the version within the service. For example, 'v1'. Version names can contain only lowercase letters, numbers, or hyphens. Reserved names,"default", "latest", and any name with the prefix "ah-".</rdfs:comment>
    <rdfs:domain rdf:resource="http://example.org/onto/class/google_app_engine_standard_app_version"/>
    <rdfs:range rdf:resource="http://www.w3.org/2001/XMLSchema#string"/>
  </owl:DatatypeProperty>
  <owl:DatatypeProperty rdf:about="http://example.org/onto/prop/google_app_engine_standard_app_version_max_concurrent_requests">
    <rdfs:label>max_concurrent_requests</rdfs:label>
    <rdfs:comment>Number of concurrent requests an automatic scaling instance can accept before the scheduler spawns a new instance.

Defaults to a runtime-specific value.</rdfs:comment>
    <rdfs:domain rdf:resource="http://example.org/onto/class/google_app_engine_standard_app_version"/>
    <rdfs:range rdf:resource="http://www.w3.org/2001/XMLSchema#string"/>
  </owl:DatatypeProperty>
  <owl:DatatypeProperty rdf:about="http://example.org/onto/prop/google_app_engine_standard_app_version_max_idle_instances">
    <rdfs:label>max_idle_instances</rdfs:label>
    <rdfs:comment>Maximum number of idle instances that should be maintained for this version.</rdfs:comment>
    <rdfs:domain rdf:resource="http://example.org/onto/class/google_app_engine_standard_app_version"/>
    <rdfs:range rdf:resource="http://www.w3.org/2001/XMLSchema#string"/>
  </owl:DatatypeProperty>
  <owl:DatatypeProperty rdf:about="http://example.org/onto/prop/google_app_engine_standard_app_version_max_pending_latency">
    <rdfs:label>max_pending_latency</rdfs:label>
    <rdfs:comment>Maximum amount of time that a request should wait in the pending queue before starting a new instance to handle it.
A duration in seconds with up to nine fractional digits, terminated by 's'. Example: "3.5s".</rdfs:comment>
    <rdfs:domain rdf:resource="http://example.org/onto/class/google_app_engine_standard_app_version"/>
    <rdfs:range rdf:resource="http://www.w3.org/2001/XMLSchema#string"/>
  </owl:DatatypeProperty>
  <owl:DatatypeProperty rdf:about="http://example.org/onto/prop/google_app_engine_standard_app_version_min_idle_instances">
    <rdfs:label>min_idle_instances</rdfs:label>
    <rdfs:comment>Minimum number of idle instances that should be maintained for this version. Only applicable for the default version of a service.</rdfs:comment>
    <rdfs:domain rdf:resource="http://example.org/onto/class/google_app_engine_standard_app_version"/>
    <rdfs:range rdf:resource="http://www.w3.org/2001/XMLSchema#string"/>
  </owl:DatatypeProperty>
  <owl:DatatypeProperty rdf:about="http://example.org/onto/prop/google_app_engine_standard_app_version_min_pending_latency">
    <rdfs:label>min_pending_latency</rdfs:label>
    <rdfs:comment>Minimum amount of time a request should wait in the pending queue before starting a new instance to handle it.
A duration in seconds with up to nine fractional digits, terminated by 's'. Example: "3.5s".</rdfs:comment>
    <rdfs:domain rdf:resource="http://example.org/onto/class/google_app_engine_standard_app_version"/>
    <rdfs:range rdf:resource="http://www.w3.org/2001/XMLSchema#string"/>
  </owl:DatatypeProperty>
  <owl:DatatypeProperty rdf:about="http://example.org/onto/prop/google_app_engine_standard_app_version_max_instances">
    <rdfs:label>max_instances</rdfs:label>
    <rdfs:comment>Maximum number of instances to run for this version. Set to zero to disable maxInstances configuration.

**Note:** Starting from March 2025, App Engine sets the maxInstances default for standard environment deployments to 20. This change doesn't impact existing apps. To override the default, specify a new value between 0 and 2147483647, and deploy a new version or redeploy over an existing version. To disable the maxInstances default configuration setting, specify the maximum permitted value 2147483647.</rdfs:comment>
    <rdfs:domain rdf:resource="http://example.org/onto/class/google_app_engine_standard_app_version"/>
    <rdfs:range rdf:resource="http://www.w3.org/2001/XMLSchema#string"/>
  </owl:DatatypeProperty>
  <owl:DatatypeProperty rdf:about="http://example.org/onto/prop/google_app_engine_standard_app_version_min_instances">
    <rdfs:label>min_instances</rdfs:label>
    <rdfs:comment>Minimum number of instances to run for this version. Set to zero to disable minInstances configuration.</rdfs:comment>
    <rdfs:domain rdf:resource="http://example.org/onto/class/google_app_engine_standard_app_version"/>
    <rdfs:range rdf:resource="http://www.w3.org/2001/XMLSchema#string"/>
  </owl:DatatypeProperty>
  <owl:DatatypeProperty rdf:about="http://example.org/onto/prop/google_app_engine_standard_app_version_target_cpu_utilization">
    <rdfs:label>target_cpu_utilization</rdfs:label>
    <rdfs:comment>Target CPU utilization ratio to maintain when scaling. Should be a value in the range [0.50, 0.95], zero, or a negative value.</rdfs:comment>
    <rdfs:domain rdf:resource="http://example.org/onto/class/google_app_engine_standard_app_version"/>
    <rdfs:range rdf:resource="http://www.w3.org/2001/XMLSchema#string"/>
  </owl:DatatypeProperty>
  <owl:DatatypeProperty rdf:about="http://example.org/onto/prop/google_app_engine_standard_app_version_target_throughput_utilization">
    <rdfs:label>target_throughput_utilization</rdfs:label>
    <rdfs:comment>Target throughput utilization ratio to maintain when scaling. Should be a value in the range [0.50, 0.95], zero, or a negative value.</rdfs:comment>
    <rdfs:domain rdf:resource="http://example.org/onto/class/google_app_engine_standard_app_version"/>
    <rdfs:range rdf:resource="http://www.w3.org/2001/XMLSchema#string"/>
  </owl:DatatypeProperty>
  <owl:DatatypeProperty rdf:about="http://example.org/onto/prop/google_app_engine_standard_app_version_idle_timeout">
    <rdfs:label>idle_timeout</rdfs:label>
    <rdfs:comment>Duration of time after the last request that an instance must wait before the instance is shut down.
A duration in seconds with up to nine fractional digits, terminated by 's'. Example: "3.5s". Defaults to 900s.</rdfs:comment>
    <rdfs:domain rdf:resource="http://example.org/onto/class/google_app_engine_standard_app_version"/>
    <rdfs:range rdf:resource="http://www.w3.org/2001/XMLSchema#string"/>
  </owl:DatatypeProperty>
  <owl:DatatypeProperty rdf:about="http://example.org/onto/prop/google_app_engine_standard_app_version_max_instances">
    <rdfs:label>max_instances</rdfs:label>
    <rdfs:comment>Maximum number of instances to create for this version. Must be in the range [1.0, 200.0].</rdfs:comment>
    <rdfs:domain rdf:resource="http://example.org/onto/class/google_app_engine_standard_app_version"/>
    <rdfs:range rdf:resource="http://www.w3.org/2001/XMLSchema#string"/>
  </owl:DatatypeProperty>
  <owl:DatatypeProperty rdf:about="http://example.org/onto/prop/google_app_engine_standard_app_version_name">
    <rdfs:label>name</rdfs:label>
    <rdfs:domain rdf:resource="http://example.org/onto/class/google_app_engine_standard_app_version"/>
    <rdfs:range rdf:resource="http://www.w3.org/2001/XMLSchema#string"/>
  </owl:DatatypeProperty>
  <owl:DatatypeProperty rdf:about="http://example.org/onto/prop/google_app_engine_standard_app_version_sha1_sum">
    <rdfs:label>sha1_sum</rdfs:label>
    <rdfs:comment>SHA1 checksum of the file</rdfs:comment>
    <rdfs:domain rdf:resource="http://example.org/onto/class/google_app_engine_standard_app_version"/>
    <rdfs:range rdf:resource="http://www.w3.org/2001/XMLSchema#string"/>
  </owl:DatatypeProperty>
  <owl:DatatypeProperty rdf:about="http://example.org/onto/prop/google_app_engine_standard_app_version_source_url">
    <rdfs:label>source_url</rdfs:label>
    <rdfs:comment>Source URL</rdfs:comment>
    <rdfs:domain rdf:resource="http://example.org/onto/class/google_app_engine_standard_app_version"/>
    <rdfs:range rdf:resource="http://www.w3.org/2001/XMLSchema#string"/>
  </owl:DatatypeProperty>
  <owl:DatatypeProperty rdf:about="http://example.org/onto/prop/google_app_engine_standard_app_version_files_count">
    <rdfs:label>files_count</rdfs:label>
    <rdfs:comment>files count</rdfs:comment>
    <rdfs:domain rdf:resource="http://example.org/onto/class/google_app_engine_standard_app_version"/>
    <rdfs:range rdf:resource="http://www.w3.org/2001/XMLSchema#string"/>
  </owl:DatatypeProperty>
  <owl:DatatypeProperty rdf:about="http://example.org/onto/prop/google_app_engine_standard_app_version_source_url">
    <rdfs:label>source_url</rdfs:label>
    <rdfs:comment>Source URL</rdfs:comment>
    <rdfs:domain rdf:resource="http://example.org/onto/class/google_app_engine_standard_app_version"/>
    <rdfs:range rdf:resource="http://www.w3.org/2001/XMLSchema#string"/>
  </owl:DatatypeProperty>
  <owl:DatatypeProperty rdf:about="http://example.org/onto/prop/google_app_engine_standard_app_version_shell">
    <rdfs:label>shell</rdfs:label>
    <rdfs:comment>The format should be a shell command that can be fed to bash -c.</rdfs:comment>
    <rdfs:domain rdf:resource="http://example.org/onto/class/google_app_engine_standard_app_version"/>
    <rdfs:range rdf:resource="http://www.w3.org/2001/XMLSchema#string"/>
  </owl:DatatypeProperty>
  <owl:DatatypeProperty rdf:about="http://example.org/onto/prop/google_app_engine_standard_app_version_auth_fail_action">
    <rdfs:label>auth_fail_action</rdfs:label>
    <rdfs:comment>Actions to take when the user is not logged in. Possible values: ["AUTH_FAIL_ACTION_REDIRECT", "AUTH_FAIL_ACTION_UNAUTHORIZED"]</rdfs:comment>
    <rdfs:domain rdf:resource="http://example.org/onto/class/google_app_engine_standard_app_version"/>
    <rdfs:range rdf:resource="http://www.w3.org/2001/XMLSchema#string"/>
  </owl:DatatypeProperty>
  <owl:DatatypeProperty rdf:about="http://example.org/onto/prop/google_app_engine_standard_app_version_login">
    <rdfs:label>login</rdfs:label>
    <rdfs:comment>Methods to restrict access to a URL based on login status. Possible values: ["LOGIN_OPTIONAL", "LOGIN_ADMIN", "LOGIN_REQUIRED"]</rdfs:comment>
    <rdfs:domain rdf:resource="http://example.org/onto/class/google_app_engine_standard_app_version"/>
    <rdfs:range rdf:resource="http://www.w3.org/2001/XMLSchema#string"/>
  </owl:DatatypeProperty>
  <owl:DatatypeProperty rdf:about="http://example.org/onto/prop/google_app_engine_standard_app_version_redirect_http_response_code">
    <rdfs:label>redirect_http_response_code</rdfs:label>
    <rdfs:comment>30x code to use when performing redirects for the secure field. Possible values: ["REDIRECT_HTTP_RESPONSE_CODE_301", "REDIRECT_HTTP_RESPONSE_CODE_302", "REDIRECT_HTTP_RESPONSE_CODE_303", "REDIRECT_HTTP_RESPONSE_CODE_307"]</rdfs:comment>
    <rdfs:domain rdf:resource="http://example.org/onto/class/google_app_engine_standard_app_version"/>
    <rdfs:range rdf:resource="http://www.w3.org/2001/XMLSchema#string"/>
  </owl:DatatypeProperty>
  <owl:DatatypeProperty rdf:about="http://example.org/onto/prop/google_app_engine_standard_app_version_security_level">
    <rdfs:label>security_level</rdfs:label>
    <rdfs:comment>Security (HTTPS) enforcement for this URL. Possible values: ["SECURE_DEFAULT", "SECURE_NEVER", "SECURE_OPTIONAL", "SECURE_ALWAYS"]</rdfs:comment>
    <rdfs:domain rdf:resource="http://example.org/onto/class/google_app_engine_standard_app_version"/>
    <rdfs:range rdf:resource="http://www.w3.org/2001/XMLSchema#string"/>
  </owl:DatatypeProperty>
  <owl:DatatypeProperty rdf:about="http://example.org/onto/prop/google_app_engine_standard_app_version_url_regex">
    <rdfs:label>url_regex</rdfs:label>
    <rdfs:comment>URL prefix. Uses regular expression syntax, which means regexp special characters must be escaped, but should not contain groupings.
All URLs that begin with this prefix are handled by this handler, using the portion of the URL after the prefix as part of the file path.</rdfs:comment>
    <rdfs:domain rdf:resource="http://example.org/onto/class/google_app_engine_standard_app_version"/>
    <rdfs:range rdf:resource="http://www.w3.org/2001/XMLSchema#string"/>
  </owl:DatatypeProperty>
  <owl:DatatypeProperty rdf:about="http://example.org/onto/prop/google_app_engine_standard_app_version_script_path">
    <rdfs:label>script_path</rdfs:label>
    <rdfs:comment>Path to the script from the application root directory.</rdfs:comment>
    <rdfs:domain rdf:resource="http://example.org/onto/class/google_app_engine_standard_app_version"/>
    <rdfs:range rdf:resource="http://www.w3.org/2001/XMLSchema#string"/>
  </owl:DatatypeProperty>
  <owl:DatatypeProperty rdf:about="http://example.org/onto/prop/google_app_engine_standard_app_version_application_readable">
    <rdfs:label>application_readable</rdfs:label>
    <rdfs:comment>Whether files should also be uploaded as code data. By default, files declared in static file handlers are uploaded as
static data and are only served to end users; they cannot be read by the application. If enabled, uploads are charged
against both your code and static data storage resource quotas.</rdfs:comment>
    <rdfs:domain rdf:resource="http://example.org/onto/class/google_app_engine_standard_app_version"/>
    <rdfs:range rdf:resource="http://www.w3.org/2001/XMLSchema#string"/>
  </owl:DatatypeProperty>
  <owl:DatatypeProperty rdf:about="http://example.org/onto/prop/google_app_engine_standard_app_version_expiration">
    <rdfs:label>expiration</rdfs:label>
    <rdfs:comment>Time a static file served by this handler should be cached by web proxies and browsers.
A duration in seconds with up to nine fractional digits, terminated by 's'. Example "3.5s".</rdfs:comment>
    <rdfs:domain rdf:resource="http://example.org/onto/class/google_app_engine_standard_app_version"/>
    <rdfs:range rdf:resource="http://www.w3.org/2001/XMLSchema#string"/>
  </owl:DatatypeProperty>
  <owl:DatatypeProperty rdf:about="http://example.org/onto/prop/google_app_engine_standard_app_version_http_headers">
    <rdfs:label>http_headers</rdfs:label>
    <rdfs:comment>HTTP headers to use for all responses from these URLs.
An object containing a list of "key:value" value pairs.".</rdfs:comment>
    <rdfs:domain rdf:resource="http://example.org/onto/class/google_app_engine_standard_app_version"/>
    <rdfs:range rdf:resource="http://www.w3.org/2001/XMLSchema#string"/>
  </owl:DatatypeProperty>
  <owl:DatatypeProperty rdf:about="http://example.org/onto/prop/google_app_engine_standard_app_version_mime_type">
    <rdfs:label>mime_type</rdfs:label>
    <rdfs:comment>MIME type used to serve all files served by this handler.
Defaults to file-specific MIME types, which are derived from each file's filename extension.</rdfs:comment>
    <rdfs:domain rdf:resource="http://example.org/onto/class/google_app_engine_standard_app_version"/>
    <rdfs:range rdf:resource="http://www.w3.org/2001/XMLSchema#string"/>
  </owl:DatatypeProperty>
  <owl:DatatypeProperty rdf:about="http://example.org/onto/prop/google_app_engine_standard_app_version_path">
    <rdfs:label>path</rdfs:label>
    <rdfs:comment>Path to the static files matched by the URL pattern, from the application root directory. The path can refer to text matched in groupings in the URL pattern.</rdfs:comment>
    <rdfs:domain rdf:resource="http://example.org/onto/class/google_app_engine_standard_app_version"/>
    <rdfs:range rdf:resource="http://www.w3.org/2001/XMLSchema#string"/>
  </owl:DatatypeProperty>
  <owl:DatatypeProperty rdf:about="http://example.org/onto/prop/google_app_engine_standard_app_version_require_matching_file">
    <rdfs:label>require_matching_file</rdfs:label>
    <rdfs:comment>Whether this handler should match the request if the file referenced by the handler does not exist.</rdfs:comment>
    <rdfs:domain rdf:resource="http://example.org/onto/class/google_app_engine_standard_app_version"/>
    <rdfs:range rdf:resource="http://www.w3.org/2001/XMLSchema#string"/>
  </owl:DatatypeProperty>
  <owl:DatatypeProperty rdf:about="http://example.org/onto/prop/google_app_engine_standard_app_version_upload_path_regex">
    <rdfs:label>upload_path_regex</rdfs:label>
    <rdfs:comment>Regular expression that matches the file paths for all files that should be referenced by this handler.</rdfs:comment>
    <rdfs:domain rdf:resource="http://example.org/onto/class/google_app_engine_standard_app_version"/>
    <rdfs:range rdf:resource="http://www.w3.org/2001/XMLSchema#string"/>
  </owl:DatatypeProperty>
  <owl:DatatypeProperty rdf:about="http://example.org/onto/prop/google_app_engine_standard_app_version_name">
    <rdfs:label>name</rdfs:label>
    <rdfs:comment>Name of the library. Example "django".</rdfs:comment>
    <rdfs:domain rdf:resource="http://example.org/onto/class/google_app_engine_standard_app_version"/>
    <rdfs:range rdf:resource="http://www.w3.org/2001/XMLSchema#string"/>
  </owl:DatatypeProperty>
  <owl:DatatypeProperty rdf:about="http://example.org/onto/prop/google_app_engine_standard_app_version_version">
    <rdfs:label>version</rdfs:label>
    <rdfs:comment>Version of the library to select, or "latest".</rdfs:comment>
    <rdfs:domain rdf:resource="http://example.org/onto/class/google_app_engine_standard_app_version"/>
    <rdfs:range rdf:resource="http://www.w3.org/2001/XMLSchema#string"/>
  </owl:DatatypeProperty>
  <owl:DatatypeProperty rdf:about="http://example.org/onto/prop/google_app_engine_standard_app_version_instances">
    <rdfs:label>instances</rdfs:label>
    <rdfs:comment>Number of instances to assign to the service at the start.

**Note:** When managing the number of instances at runtime through the App Engine Admin API or the (now deprecated) Python 2
Modules API set_num_instances() you must use 'lifecycle.ignore_changes = ["manual_scaling"[0].instances]' to prevent drift detection.</rdfs:comment>
    <rdfs:domain rdf:resource="http://example.org/onto/class/google_app_engine_standard_app_version"/>
    <rdfs:range rdf:resource="http://www.w3.org/2001/XMLSchema#string"/>
  </owl:DatatypeProperty>
  <owl:DatatypeProperty rdf:about="http://example.org/onto/prop/google_app_engine_standard_app_version_create">
    <rdfs:label>create</rdfs:label>
    <rdfs:domain rdf:resource="http://example.org/onto/class/google_app_engine_standard_app_version"/>
    <rdfs:range rdf:resource="http://www.w3.org/2001/XMLSchema#string"/>
  </owl:DatatypeProperty>
  <owl:DatatypeProperty rdf:about="http://example.org/onto/prop/google_app_engine_standard_app_version_delete">
    <rdfs:label>delete</rdfs:label>
    <rdfs:domain rdf:resource="http://example.org/onto/class/google_app_engine_standard_app_version"/>
    <rdfs:range rdf:resource="http://www.w3.org/2001/XMLSchema#string"/>
  </owl:DatatypeProperty>
  <owl:DatatypeProperty rdf:about="http://example.org/onto/prop/google_app_engine_standard_app_version_update">
    <rdfs:label>update</rdfs:label>
    <rdfs:domain rdf:resource="http://example.org/onto/class/google_app_engine_standard_app_version"/>
    <rdfs:range rdf:resource="http://www.w3.org/2001/XMLSchema#string"/>
  </owl:DatatypeProperty>
  <owl:DatatypeProperty rdf:about="http://example.org/onto/prop/google_app_engine_standard_app_version_egress_setting">
    <rdfs:label>egress_setting</rdfs:label>
    <rdfs:comment>The egress setting for the connector, controlling what traffic is diverted through it.</rdfs:comment>
    <rdfs:domain rdf:resource="http://example.org/onto/class/google_app_engine_standard_app_version"/>
    <rdfs:range rdf:resource="http://www.w3.org/2001/XMLSchema#string"/>
  </owl:DatatypeProperty>
  <owl:DatatypeProperty rdf:about="http://example.org/onto/prop/google_app_engine_standard_app_version_name">
    <rdfs:label>name</rdfs:label>
    <rdfs:comment>Full Serverless VPC Access Connector name e.g. /projects/my-project/locations/us-central1/connectors/c1.</rdfs:comment>
    <rdfs:domain rdf:resource="http://example.org/onto/class/google_app_engine_standard_app_version"/>
    <rdfs:range rdf:resource="http://www.w3.org/2001/XMLSchema#string"/>
  </owl:DatatypeProperty>
</rdf:RDF>
