<?xml version="1.0" encoding="UTF-8"?>
<rdf:RDF
  xmlns:rdf="http://www.w3.org/1999/02/22-rdf-syntax-ns#"
  xmlns:rdfs="http://www.w3.org/2000/01/rdf-schema#"
  xmlns:owl="http://www.w3.org/2002/07/owl#"
  xmlns:xsd="http://www.w3.org/2001/XMLSchema#"
  xml:base="http://example.org/onto/">
  <owl:Class rdf:about="http://example.org/onto/class/google_filestore_instance">
    <rdfs:label>google_filestore_instance</rdfs:label>
    <rdfs:comment>#
#     ***     AUTO GENERATED CODE    ***    Type: MMv1     ***
#
# ----------------------------------------------------------------------------
#
#     This code is generated by Magic Modules using the following:
#
#     Configuration: https:#github.com/GoogleCloudPlatform/magic-modules/tree/main/mmv1/products/filestore/Instance.yaml
#     Template:      https:#github.com/GoogleCloudPlatform/magic-modules/tree/main/mmv1/templates/terraform/resource.html.markdown.tmpl
#
#     DO NOT EDIT this file directly. Any changes made to this file will be
#     overwritten during the next generation cycle.
#
# ----------------------------------------------------------------------------
subcategory: "Filestore"
description: |-
  A Google Cloud Filestore instance.
---</rdfs:comment>
  </owl:Class>
  <owl:DatatypeProperty rdf:about="http://example.org/onto/prop/google_filestore_instance_create_time">
    <rdfs:label>create_time</rdfs:label>
    <rdfs:comment>Creation timestamp in RFC3339 text format.</rdfs:comment>
    <rdfs:domain rdf:resource="http://example.org/onto/class/google_filestore_instance"/>
    <rdfs:range rdf:resource="http://www.w3.org/2001/XMLSchema#string"/>
  </owl:DatatypeProperty>
  <owl:DatatypeProperty rdf:about="http://example.org/onto/prop/google_filestore_instance_deletion_protection_enabled">
    <rdfs:label>deletion_protection_enabled</rdfs:label>
    <rdfs:comment>Indicates whether the instance is protected against deletion.</rdfs:comment>
    <rdfs:domain rdf:resource="http://example.org/onto/class/google_filestore_instance"/>
    <rdfs:range rdf:resource="http://www.w3.org/2001/XMLSchema#string"/>
  </owl:DatatypeProperty>
  <owl:DatatypeProperty rdf:about="http://example.org/onto/prop/google_filestore_instance_deletion_protection_reason">
    <rdfs:label>deletion_protection_reason</rdfs:label>
    <rdfs:comment>The reason for enabling deletion protection.</rdfs:comment>
    <rdfs:domain rdf:resource="http://example.org/onto/class/google_filestore_instance"/>
    <rdfs:range rdf:resource="http://www.w3.org/2001/XMLSchema#string"/>
  </owl:DatatypeProperty>
  <owl:DatatypeProperty rdf:about="http://example.org/onto/prop/google_filestore_instance_description">
    <rdfs:label>description</rdfs:label>
    <rdfs:comment>A description of the instance.</rdfs:comment>
    <rdfs:domain rdf:resource="http://example.org/onto/class/google_filestore_instance"/>
    <rdfs:range rdf:resource="http://www.w3.org/2001/XMLSchema#string"/>
  </owl:DatatypeProperty>
  <owl:DatatypeProperty rdf:about="http://example.org/onto/prop/google_filestore_instance_effective_labels">
    <rdfs:label>effective_labels</rdfs:label>
    <rdfs:comment>All of labels (key/value pairs) present on the resource in GCP, including the labels configured through Terraform, other clients and services.</rdfs:comment>
    <rdfs:domain rdf:resource="http://example.org/onto/class/google_filestore_instance"/>
    <rdfs:range rdf:resource="http://www.w3.org/2001/XMLSchema#string"/>
  </owl:DatatypeProperty>
  <owl:DatatypeProperty rdf:about="http://example.org/onto/prop/google_filestore_instance_effective_replication">
    <rdfs:label>effective_replication</rdfs:label>
    <rdfs:comment>Output only fields for replication configuration.</rdfs:comment>
    <rdfs:domain rdf:resource="http://example.org/onto/class/google_filestore_instance"/>
    <rdfs:range rdf:resource="http://www.w3.org/2001/XMLSchema#string"/>
  </owl:DatatypeProperty>
  <owl:DatatypeProperty rdf:about="http://example.org/onto/prop/google_filestore_instance_etag">
    <rdfs:label>etag</rdfs:label>
    <rdfs:comment>Server-specified ETag for the instance resource to prevent
simultaneous updates from overwriting each other.</rdfs:comment>
    <rdfs:domain rdf:resource="http://example.org/onto/class/google_filestore_instance"/>
    <rdfs:range rdf:resource="http://www.w3.org/2001/XMLSchema#string"/>
  </owl:DatatypeProperty>
  <owl:DatatypeProperty rdf:about="http://example.org/onto/prop/google_filestore_instance_id">
    <rdfs:label>id</rdfs:label>
    <rdfs:domain rdf:resource="http://example.org/onto/class/google_filestore_instance"/>
    <rdfs:range rdf:resource="http://www.w3.org/2001/XMLSchema#string"/>
  </owl:DatatypeProperty>
  <owl:DatatypeProperty rdf:about="http://example.org/onto/prop/google_filestore_instance_kms_key_name">
    <rdfs:label>kms_key_name</rdfs:label>
    <rdfs:comment>KMS key name used for data encryption.</rdfs:comment>
    <rdfs:domain rdf:resource="http://example.org/onto/class/google_filestore_instance"/>
    <rdfs:range rdf:resource="http://www.w3.org/2001/XMLSchema#string"/>
  </owl:DatatypeProperty>
  <owl:DatatypeProperty rdf:about="http://example.org/onto/prop/google_filestore_instance_labels">
    <rdfs:label>labels</rdfs:label>
    <rdfs:comment>Resource labels to represent user-provided metadata.


**Note**: This field is non-authoritative, and will only manage the labels present in your configuration.
Please refer to the field 'effective_labels' for all of the labels present on the resource.</rdfs:comment>
    <rdfs:domain rdf:resource="http://example.org/onto/class/google_filestore_instance"/>
    <rdfs:range rdf:resource="http://www.w3.org/2001/XMLSchema#string"/>
  </owl:DatatypeProperty>
  <owl:DatatypeProperty rdf:about="http://example.org/onto/prop/google_filestore_instance_location">
    <rdfs:label>location</rdfs:label>
    <rdfs:comment>The name of the location of the instance. This can be a region for ENTERPRISE tier instances.</rdfs:comment>
    <rdfs:domain rdf:resource="http://example.org/onto/class/google_filestore_instance"/>
    <rdfs:range rdf:resource="http://www.w3.org/2001/XMLSchema#string"/>
  </owl:DatatypeProperty>
  <owl:DatatypeProperty rdf:about="http://example.org/onto/prop/google_filestore_instance_name">
    <rdfs:label>name</rdfs:label>
    <rdfs:comment>The resource name of the instance.</rdfs:comment>
    <rdfs:domain rdf:resource="http://example.org/onto/class/google_filestore_instance"/>
    <rdfs:range rdf:resource="http://www.w3.org/2001/XMLSchema#string"/>
  </owl:DatatypeProperty>
  <owl:DatatypeProperty rdf:about="http://example.org/onto/prop/google_filestore_instance_project">
    <rdfs:label>project</rdfs:label>
    <rdfs:domain rdf:resource="http://example.org/onto/class/google_filestore_instance"/>
    <rdfs:range rdf:resource="http://www.w3.org/2001/XMLSchema#string"/>
  </owl:DatatypeProperty>
  <owl:DatatypeProperty rdf:about="http://example.org/onto/prop/google_filestore_instance_protocol">
    <rdfs:label>protocol</rdfs:label>
    <rdfs:comment>Either NFSv3, for using NFS version 3 as file sharing protocol,
or NFSv4.1, for using NFS version 4.1 as file sharing protocol.
NFSv4.1 can be used with HIGH_SCALE_SSD, ZONAL, REGIONAL and ENTERPRISE.
The default is NFSv3. Default value: "NFS_V3" Possible values: ["NFS_V3", "NFS_V4_1"]</rdfs:comment>
    <rdfs:domain rdf:resource="http://example.org/onto/class/google_filestore_instance"/>
    <rdfs:range rdf:resource="http://www.w3.org/2001/XMLSchema#string"/>
  </owl:DatatypeProperty>
  <owl:DatatypeProperty rdf:about="http://example.org/onto/prop/google_filestore_instance_tags">
    <rdfs:label>tags</rdfs:label>
    <rdfs:comment>A map of resource manager tags. Resource manager tag keys
and values have the same definition as resource manager
tags. Keys must be in the format tagKeys/{tag_key_id},
and values are in the format tagValues/456. The field is
ignored when empty. The field is immutable and causes
resource replacement when mutated. This field is only set
at create time and modifying this field after creation
will trigger recreation. To apply tags to an existing
resource, see the 'google_tags_tag_value' resource.</rdfs:comment>
    <rdfs:domain rdf:resource="http://example.org/onto/class/google_filestore_instance"/>
    <rdfs:range rdf:resource="http://www.w3.org/2001/XMLSchema#string"/>
  </owl:DatatypeProperty>
  <owl:DatatypeProperty rdf:about="http://example.org/onto/prop/google_filestore_instance_terraform_labels">
    <rdfs:label>terraform_labels</rdfs:label>
    <rdfs:comment>The combination of labels configured directly on the resource
 and default labels configured on the provider.</rdfs:comment>
    <rdfs:domain rdf:resource="http://example.org/onto/class/google_filestore_instance"/>
    <rdfs:range rdf:resource="http://www.w3.org/2001/XMLSchema#string"/>
  </owl:DatatypeProperty>
  <owl:DatatypeProperty rdf:about="http://example.org/onto/prop/google_filestore_instance_tier">
    <rdfs:label>tier</rdfs:label>
    <rdfs:comment>The service tier of the instance.
Possible values include: STANDARD, PREMIUM, BASIC_HDD, BASIC_SSD, HIGH_SCALE_SSD, ZONAL, REGIONAL and ENTERPRISE</rdfs:comment>
    <rdfs:domain rdf:resource="http://example.org/onto/class/google_filestore_instance"/>
    <rdfs:range rdf:resource="http://www.w3.org/2001/XMLSchema#string"/>
  </owl:DatatypeProperty>
  <owl:DatatypeProperty rdf:about="http://example.org/onto/prop/google_filestore_instance_zone">
    <rdfs:label>zone</rdfs:label>
    <rdfs:comment>The name of the Filestore zone of the instance.</rdfs:comment>
    <rdfs:domain rdf:resource="http://example.org/onto/class/google_filestore_instance"/>
    <rdfs:range rdf:resource="http://www.w3.org/2001/XMLSchema#string"/>
  </owl:DatatypeProperty>
  <owl:DatatypeProperty rdf:about="http://example.org/onto/prop/google_filestore_instance_capacity_gb">
    <rdfs:label>capacity_gb</rdfs:label>
    <rdfs:comment>File share capacity in GiB. This must be at least 1024 GiB
for the standard tier, or 2560 GiB for the premium tier.</rdfs:comment>
    <rdfs:domain rdf:resource="http://example.org/onto/class/google_filestore_instance"/>
    <rdfs:range rdf:resource="http://www.w3.org/2001/XMLSchema#string"/>
  </owl:DatatypeProperty>
  <owl:DatatypeProperty rdf:about="http://example.org/onto/prop/google_filestore_instance_name">
    <rdfs:label>name</rdfs:label>
    <rdfs:comment>The name of the fileshare (16 characters or less)</rdfs:comment>
    <rdfs:domain rdf:resource="http://example.org/onto/class/google_filestore_instance"/>
    <rdfs:range rdf:resource="http://www.w3.org/2001/XMLSchema#string"/>
  </owl:DatatypeProperty>
  <owl:DatatypeProperty rdf:about="http://example.org/onto/prop/google_filestore_instance_source_backup">
    <rdfs:label>source_backup</rdfs:label>
    <rdfs:comment>The resource name of the backup, in the format
projects/{projectId}/locations/{locationId}/backups/{backupId},
that this file share has been restored from.</rdfs:comment>
    <rdfs:domain rdf:resource="http://example.org/onto/class/google_filestore_instance"/>
    <rdfs:range rdf:resource="http://www.w3.org/2001/XMLSchema#string"/>
  </owl:DatatypeProperty>
  <owl:DatatypeProperty rdf:about="http://example.org/onto/prop/google_filestore_instance_access_mode">
    <rdfs:label>access_mode</rdfs:label>
    <rdfs:comment>Either READ_ONLY, for allowing only read requests on the exported directory,
or READ_WRITE, for allowing both read and write requests. The default is READ_WRITE. Default value: "READ_WRITE" Possible values: ["READ_ONLY", "READ_WRITE"]</rdfs:comment>
    <rdfs:domain rdf:resource="http://example.org/onto/class/google_filestore_instance"/>
    <rdfs:range rdf:resource="http://www.w3.org/2001/XMLSchema#string"/>
  </owl:DatatypeProperty>
  <owl:DatatypeProperty rdf:about="http://example.org/onto/prop/google_filestore_instance_anon_gid">
    <rdfs:label>anon_gid</rdfs:label>
    <rdfs:comment>An integer representing the anonymous group id with a default value of 65534.
Anon_gid may only be set with squashMode of ROOT_SQUASH. An error will be returned
if this field is specified for other squashMode settings.</rdfs:comment>
    <rdfs:domain rdf:resource="http://example.org/onto/class/google_filestore_instance"/>
    <rdfs:range rdf:resource="http://www.w3.org/2001/XMLSchema#string"/>
  </owl:DatatypeProperty>
  <owl:DatatypeProperty rdf:about="http://example.org/onto/prop/google_filestore_instance_anon_uid">
    <rdfs:label>anon_uid</rdfs:label>
    <rdfs:comment>An integer representing the anonymous user id with a default value of 65534.
Anon_uid may only be set with squashMode of ROOT_SQUASH. An error will be returned
if this field is specified for other squashMode settings.</rdfs:comment>
    <rdfs:domain rdf:resource="http://example.org/onto/class/google_filestore_instance"/>
    <rdfs:range rdf:resource="http://www.w3.org/2001/XMLSchema#string"/>
  </owl:DatatypeProperty>
  <owl:DatatypeProperty rdf:about="http://example.org/onto/prop/google_filestore_instance_ip_ranges">
    <rdfs:label>ip_ranges</rdfs:label>
    <rdfs:comment>List of either IPv4 addresses, or ranges in CIDR notation which may mount the file share.
Overlapping IP ranges are not allowed, both within and across NfsExportOptions. An error will be returned.
The limit is 64 IP ranges/addresses for each FileShareConfig among all NfsExportOptions.</rdfs:comment>
    <rdfs:domain rdf:resource="http://example.org/onto/class/google_filestore_instance"/>
    <rdfs:range rdf:resource="http://www.w3.org/2001/XMLSchema#string"/>
  </owl:DatatypeProperty>
  <owl:DatatypeProperty rdf:about="http://example.org/onto/prop/google_filestore_instance_network">
    <rdfs:label>network</rdfs:label>
    <rdfs:comment>The source VPC network for 'ip_ranges'.
Required for instances using Private Service Connect, optional otherwise.</rdfs:comment>
    <rdfs:domain rdf:resource="http://example.org/onto/class/google_filestore_instance"/>
    <rdfs:range rdf:resource="http://www.w3.org/2001/XMLSchema#string"/>
  </owl:DatatypeProperty>
  <owl:DatatypeProperty rdf:about="http://example.org/onto/prop/google_filestore_instance_squash_mode">
    <rdfs:label>squash_mode</rdfs:label>
    <rdfs:comment>Either NO_ROOT_SQUASH, for allowing root access on the exported directory, or ROOT_SQUASH,
for not allowing root access. The default is NO_ROOT_SQUASH. Default value: "NO_ROOT_SQUASH" Possible values: ["NO_ROOT_SQUASH", "ROOT_SQUASH"]</rdfs:comment>
    <rdfs:domain rdf:resource="http://example.org/onto/class/google_filestore_instance"/>
    <rdfs:range rdf:resource="http://www.w3.org/2001/XMLSchema#string"/>
  </owl:DatatypeProperty>
  <owl:DatatypeProperty rdf:about="http://example.org/onto/prop/google_filestore_instance_role">
    <rdfs:label>role</rdfs:label>
    <rdfs:comment>The replication role. Default value: "STANDBY" Possible values: ["ROLE_UNSPECIFIED", "ACTIVE", "STANDBY"]</rdfs:comment>
    <rdfs:domain rdf:resource="http://example.org/onto/class/google_filestore_instance"/>
    <rdfs:range rdf:resource="http://www.w3.org/2001/XMLSchema#string"/>
  </owl:DatatypeProperty>
  <owl:DatatypeProperty rdf:about="http://example.org/onto/prop/google_filestore_instance_peer_instance">
    <rdfs:label>peer_instance</rdfs:label>
    <rdfs:comment>The peer instance.</rdfs:comment>
    <rdfs:domain rdf:resource="http://example.org/onto/class/google_filestore_instance"/>
    <rdfs:range rdf:resource="http://www.w3.org/2001/XMLSchema#string"/>
  </owl:DatatypeProperty>
  <owl:DatatypeProperty rdf:about="http://example.org/onto/prop/google_filestore_instance_connect_mode">
    <rdfs:label>connect_mode</rdfs:label>
    <rdfs:comment>The network connect mode of the Filestore instance.
If not provided, the connect mode defaults to
DIRECT_PEERING. Default value: "DIRECT_PEERING" Possible values: ["DIRECT_PEERING", "PRIVATE_SERVICE_ACCESS", "PRIVATE_SERVICE_CONNECT"]</rdfs:comment>
    <rdfs:domain rdf:resource="http://example.org/onto/class/google_filestore_instance"/>
    <rdfs:range rdf:resource="http://www.w3.org/2001/XMLSchema#string"/>
  </owl:DatatypeProperty>
  <owl:DatatypeProperty rdf:about="http://example.org/onto/prop/google_filestore_instance_ip_addresses">
    <rdfs:label>ip_addresses</rdfs:label>
    <rdfs:comment>A list of IPv4 or IPv6 addresses.</rdfs:comment>
    <rdfs:domain rdf:resource="http://example.org/onto/class/google_filestore_instance"/>
    <rdfs:range rdf:resource="http://www.w3.org/2001/XMLSchema#string"/>
  </owl:DatatypeProperty>
  <owl:DatatypeProperty rdf:about="http://example.org/onto/prop/google_filestore_instance_modes">
    <rdfs:label>modes</rdfs:label>
    <rdfs:comment>IP versions for which the instance has
IP addresses assigned. Possible values: ["ADDRESS_MODE_UNSPECIFIED", "MODE_IPV4", "MODE_IPV6"]</rdfs:comment>
    <rdfs:domain rdf:resource="http://example.org/onto/class/google_filestore_instance"/>
    <rdfs:range rdf:resource="http://www.w3.org/2001/XMLSchema#string"/>
  </owl:DatatypeProperty>
  <owl:DatatypeProperty rdf:about="http://example.org/onto/prop/google_filestore_instance_network">
    <rdfs:label>network</rdfs:label>
    <rdfs:comment>The name of the GCE VPC network to which the
instance is connected.</rdfs:comment>
    <rdfs:domain rdf:resource="http://example.org/onto/class/google_filestore_instance"/>
    <rdfs:range rdf:resource="http://www.w3.org/2001/XMLSchema#string"/>
  </owl:DatatypeProperty>
  <owl:DatatypeProperty rdf:about="http://example.org/onto/prop/google_filestore_instance_reserved_ip_range">
    <rdfs:label>reserved_ip_range</rdfs:label>
    <rdfs:comment>A /29 CIDR block that identifies the range of IP
addresses reserved for this instance.</rdfs:comment>
    <rdfs:domain rdf:resource="http://example.org/onto/class/google_filestore_instance"/>
    <rdfs:range rdf:resource="http://www.w3.org/2001/XMLSchema#string"/>
  </owl:DatatypeProperty>
  <owl:DatatypeProperty rdf:about="http://example.org/onto/prop/google_filestore_instance_endpoint_project">
    <rdfs:label>endpoint_project</rdfs:label>
    <rdfs:comment>Consumer service project in which the Private Service Connect endpoint
would be set up. This is optional, and only relevant in case the network
is a shared VPC. If this is not specified, the endpoint would be set up
in the VPC host project.</rdfs:comment>
    <rdfs:domain rdf:resource="http://example.org/onto/class/google_filestore_instance"/>
    <rdfs:range rdf:resource="http://www.w3.org/2001/XMLSchema#string"/>
  </owl:DatatypeProperty>
  <owl:DatatypeProperty rdf:about="http://example.org/onto/prop/google_filestore_instance_max_iops">
    <rdfs:label>max_iops</rdfs:label>
    <rdfs:comment>The number of IOPS to provision for the instance.
max_iops must be in multiple of 1000.</rdfs:comment>
    <rdfs:domain rdf:resource="http://example.org/onto/class/google_filestore_instance"/>
    <rdfs:range rdf:resource="http://www.w3.org/2001/XMLSchema#string"/>
  </owl:DatatypeProperty>
  <owl:DatatypeProperty rdf:about="http://example.org/onto/prop/google_filestore_instance_max_iops_per_tb">
    <rdfs:label>max_iops_per_tb</rdfs:label>
    <rdfs:comment>The instance max IOPS will be calculated by multiplying
the capacity of the instance (TB) by max_iops_per_tb,
and rounding to the nearest 1000. The instance max IOPS
will be changed dynamically based on the instance
capacity.</rdfs:comment>
    <rdfs:domain rdf:resource="http://example.org/onto/class/google_filestore_instance"/>
    <rdfs:range rdf:resource="http://www.w3.org/2001/XMLSchema#string"/>
  </owl:DatatypeProperty>
  <owl:DatatypeProperty rdf:about="http://example.org/onto/prop/google_filestore_instance_create">
    <rdfs:label>create</rdfs:label>
    <rdfs:domain rdf:resource="http://example.org/onto/class/google_filestore_instance"/>
    <rdfs:range rdf:resource="http://www.w3.org/2001/XMLSchema#string"/>
  </owl:DatatypeProperty>
  <owl:DatatypeProperty rdf:about="http://example.org/onto/prop/google_filestore_instance_delete">
    <rdfs:label>delete</rdfs:label>
    <rdfs:domain rdf:resource="http://example.org/onto/class/google_filestore_instance"/>
    <rdfs:range rdf:resource="http://www.w3.org/2001/XMLSchema#string"/>
  </owl:DatatypeProperty>
  <owl:DatatypeProperty rdf:about="http://example.org/onto/prop/google_filestore_instance_update">
    <rdfs:label>update</rdfs:label>
    <rdfs:domain rdf:resource="http://example.org/onto/class/google_filestore_instance"/>
    <rdfs:range rdf:resource="http://www.w3.org/2001/XMLSchema#string"/>
  </owl:DatatypeProperty>
</rdf:RDF>
