<?xml version="1.0" encoding="UTF-8"?>
<rdf:RDF
  xmlns:rdf="http://www.w3.org/1999/02/22-rdf-syntax-ns#"
  xmlns:rdfs="http://www.w3.org/2000/01/rdf-schema#"
  xmlns:owl="http://www.w3.org/2002/07/owl#"
  xmlns:xsd="http://www.w3.org/2001/XMLSchema#"
  xml:base="http://example.org/onto/">
  <owl:Class rdf:about="http://example.org/onto/class/google_cloud_run_v2_service">
    <rdfs:label>google_cloud_run_v2_service</rdfs:label>
    <rdfs:comment>#
#     ***     AUTO GENERATED CODE    ***    Type: MMv1     ***
#
# ----------------------------------------------------------------------------
#
#     This code is generated by Magic Modules using the following:
#
#     Configuration: https:#github.com/GoogleCloudPlatform/magic-modules/tree/main/mmv1/products/cloudrunv2/Service.yaml
#     Template:      https:#github.com/GoogleCloudPlatform/magic-modules/tree/main/mmv1/templates/terraform/resource.html.markdown.tmpl
#
#     DO NOT EDIT this file directly. Any changes made to this file will be
#     overwritten during the next generation cycle.
#
# ----------------------------------------------------------------------------
subcategory: "Cloud Run (v2 API)"
description: |-
  Service acts as a top-level container that manages a set of configurations and revision templates which implement a network service.
---</rdfs:comment>
  </owl:Class>
  <owl:DatatypeProperty rdf:about="http://example.org/onto/prop/google_cloud_run_v2_service_annotations">
    <rdfs:label>annotations</rdfs:label>
    <rdfs:comment>Unstructured key value map that may be set by external tools to store and arbitrary metadata. They are not queryable and should be preserved when modifying objects.

Cloud Run API v2 does not support annotations with 'run.googleapis.com', 'cloud.googleapis.com', 'serving.knative.dev', or 'autoscaling.knative.dev' namespaces, and they will be rejected in new resources.
All system annotations in v1 now have a corresponding field in v2 Service.

This field follows Kubernetes annotations' namespacing, limits, and rules.

**Note**: This field is non-authoritative, and will only manage the annotations present in your configuration.
Please refer to the field 'effective_annotations' for all of the annotations present on the resource.</rdfs:comment>
    <rdfs:domain rdf:resource="http://example.org/onto/class/google_cloud_run_v2_service"/>
    <rdfs:range rdf:resource="http://www.w3.org/2001/XMLSchema#string"/>
  </owl:DatatypeProperty>
  <owl:DatatypeProperty rdf:about="http://example.org/onto/prop/google_cloud_run_v2_service_client">
    <rdfs:label>client</rdfs:label>
    <rdfs:comment>Arbitrary identifier for the API client.</rdfs:comment>
    <rdfs:domain rdf:resource="http://example.org/onto/class/google_cloud_run_v2_service"/>
    <rdfs:range rdf:resource="http://www.w3.org/2001/XMLSchema#string"/>
  </owl:DatatypeProperty>
  <owl:DatatypeProperty rdf:about="http://example.org/onto/prop/google_cloud_run_v2_service_client_version">
    <rdfs:label>client_version</rdfs:label>
    <rdfs:comment>Arbitrary version identifier for the API client.</rdfs:comment>
    <rdfs:domain rdf:resource="http://example.org/onto/class/google_cloud_run_v2_service"/>
    <rdfs:range rdf:resource="http://www.w3.org/2001/XMLSchema#string"/>
  </owl:DatatypeProperty>
  <owl:DatatypeProperty rdf:about="http://example.org/onto/prop/google_cloud_run_v2_service_conditions">
    <rdfs:label>conditions</rdfs:label>
    <rdfs:comment>The Conditions of all other associated sub-resources. They contain additional diagnostics information in case the Service does not reach its Serving state. See comments in reconciling for additional information on reconciliation process in Cloud Run.</rdfs:comment>
    <rdfs:domain rdf:resource="http://example.org/onto/class/google_cloud_run_v2_service"/>
    <rdfs:range rdf:resource="http://www.w3.org/2001/XMLSchema#string"/>
  </owl:DatatypeProperty>
  <owl:DatatypeProperty rdf:about="http://example.org/onto/prop/google_cloud_run_v2_service_create_time">
    <rdfs:label>create_time</rdfs:label>
    <rdfs:comment>The creation time.</rdfs:comment>
    <rdfs:domain rdf:resource="http://example.org/onto/class/google_cloud_run_v2_service"/>
    <rdfs:range rdf:resource="http://www.w3.org/2001/XMLSchema#string"/>
  </owl:DatatypeProperty>
  <owl:DatatypeProperty rdf:about="http://example.org/onto/prop/google_cloud_run_v2_service_creator">
    <rdfs:label>creator</rdfs:label>
    <rdfs:comment>Email address of the authenticated creator.</rdfs:comment>
    <rdfs:domain rdf:resource="http://example.org/onto/class/google_cloud_run_v2_service"/>
    <rdfs:range rdf:resource="http://www.w3.org/2001/XMLSchema#string"/>
  </owl:DatatypeProperty>
  <owl:DatatypeProperty rdf:about="http://example.org/onto/prop/google_cloud_run_v2_service_custom_audiences">
    <rdfs:label>custom_audiences</rdfs:label>
    <rdfs:comment>One or more custom audiences that you want this service to support. Specify each custom audience as the full URL in a string. The custom audiences are encoded in the token and used to authenticate requests.
For more information, see https://cloud.google.com/run/docs/configuring/custom-audiences.</rdfs:comment>
    <rdfs:domain rdf:resource="http://example.org/onto/class/google_cloud_run_v2_service"/>
    <rdfs:range rdf:resource="http://www.w3.org/2001/XMLSchema#string"/>
  </owl:DatatypeProperty>
  <owl:DatatypeProperty rdf:about="http://example.org/onto/prop/google_cloud_run_v2_service_default_uri_disabled">
    <rdfs:label>default_uri_disabled</rdfs:label>
    <rdfs:comment>Disables public resolution of the default URI of this service.</rdfs:comment>
    <rdfs:domain rdf:resource="http://example.org/onto/class/google_cloud_run_v2_service"/>
    <rdfs:range rdf:resource="http://www.w3.org/2001/XMLSchema#string"/>
  </owl:DatatypeProperty>
  <owl:DatatypeProperty rdf:about="http://example.org/onto/prop/google_cloud_run_v2_service_delete_time">
    <rdfs:label>delete_time</rdfs:label>
    <rdfs:comment>The deletion time.</rdfs:comment>
    <rdfs:domain rdf:resource="http://example.org/onto/class/google_cloud_run_v2_service"/>
    <rdfs:range rdf:resource="http://www.w3.org/2001/XMLSchema#string"/>
  </owl:DatatypeProperty>
  <owl:DatatypeProperty rdf:about="http://example.org/onto/prop/google_cloud_run_v2_service_deletion_protection">
    <rdfs:label>deletion_protection</rdfs:label>
    <rdfs:comment>Whether Terraform will be prevented from destroying the service. Defaults to true.
When a'terraform destroy' or 'terraform apply' would delete the service,
the command will fail if this field is not set to false in Terraform state.
When the field is set to true or unset in Terraform state, a 'terraform apply'
or 'terraform destroy' that would delete the service will fail.
When the field is set to false, deleting the service is allowed.</rdfs:comment>
    <rdfs:domain rdf:resource="http://example.org/onto/class/google_cloud_run_v2_service"/>
    <rdfs:range rdf:resource="http://www.w3.org/2001/XMLSchema#string"/>
  </owl:DatatypeProperty>
  <owl:DatatypeProperty rdf:about="http://example.org/onto/prop/google_cloud_run_v2_service_description">
    <rdfs:label>description</rdfs:label>
    <rdfs:comment>User-provided description of the Service. This field currently has a 512-character limit.</rdfs:comment>
    <rdfs:domain rdf:resource="http://example.org/onto/class/google_cloud_run_v2_service"/>
    <rdfs:range rdf:resource="http://www.w3.org/2001/XMLSchema#string"/>
  </owl:DatatypeProperty>
  <owl:DatatypeProperty rdf:about="http://example.org/onto/prop/google_cloud_run_v2_service_effective_annotations">
    <rdfs:label>effective_annotations</rdfs:label>
    <rdfs:comment>All of annotations (key/value pairs) present on the resource in GCP, including the annotations configured through Terraform, other clients and services.</rdfs:comment>
    <rdfs:domain rdf:resource="http://example.org/onto/class/google_cloud_run_v2_service"/>
    <rdfs:range rdf:resource="http://www.w3.org/2001/XMLSchema#string"/>
  </owl:DatatypeProperty>
  <owl:DatatypeProperty rdf:about="http://example.org/onto/prop/google_cloud_run_v2_service_effective_labels">
    <rdfs:label>effective_labels</rdfs:label>
    <rdfs:comment>All of labels (key/value pairs) present on the resource in GCP, including the labels configured through Terraform, other clients and services.</rdfs:comment>
    <rdfs:domain rdf:resource="http://example.org/onto/class/google_cloud_run_v2_service"/>
    <rdfs:range rdf:resource="http://www.w3.org/2001/XMLSchema#string"/>
  </owl:DatatypeProperty>
  <owl:DatatypeProperty rdf:about="http://example.org/onto/prop/google_cloud_run_v2_service_etag">
    <rdfs:label>etag</rdfs:label>
    <rdfs:comment>A system-generated fingerprint for this version of the resource. May be used to detect modification conflict during updates.</rdfs:comment>
    <rdfs:domain rdf:resource="http://example.org/onto/class/google_cloud_run_v2_service"/>
    <rdfs:range rdf:resource="http://www.w3.org/2001/XMLSchema#string"/>
  </owl:DatatypeProperty>
  <owl:DatatypeProperty rdf:about="http://example.org/onto/prop/google_cloud_run_v2_service_expire_time">
    <rdfs:label>expire_time</rdfs:label>
    <rdfs:comment>For a deleted resource, the time after which it will be permanently deleted.</rdfs:comment>
    <rdfs:domain rdf:resource="http://example.org/onto/class/google_cloud_run_v2_service"/>
    <rdfs:range rdf:resource="http://www.w3.org/2001/XMLSchema#string"/>
  </owl:DatatypeProperty>
  <owl:DatatypeProperty rdf:about="http://example.org/onto/prop/google_cloud_run_v2_service_generation">
    <rdfs:label>generation</rdfs:label>
    <rdfs:comment>A number that monotonically increases every time the user modifies the desired state. Please note that unlike v1, this is an int64 value. As with most Google APIs, its JSON representation will be a string instead of an integer.</rdfs:comment>
    <rdfs:domain rdf:resource="http://example.org/onto/class/google_cloud_run_v2_service"/>
    <rdfs:range rdf:resource="http://www.w3.org/2001/XMLSchema#string"/>
  </owl:DatatypeProperty>
  <owl:DatatypeProperty rdf:about="http://example.org/onto/prop/google_cloud_run_v2_service_id">
    <rdfs:label>id</rdfs:label>
    <rdfs:domain rdf:resource="http://example.org/onto/class/google_cloud_run_v2_service"/>
    <rdfs:range rdf:resource="http://www.w3.org/2001/XMLSchema#string"/>
  </owl:DatatypeProperty>
  <owl:DatatypeProperty rdf:about="http://example.org/onto/prop/google_cloud_run_v2_service_ingress">
    <rdfs:label>ingress</rdfs:label>
    <rdfs:comment>Provides the ingress settings for this Service. On output, returns the currently observed ingress settings, or INGRESS_TRAFFIC_UNSPECIFIED if no revision is active. Possible values: ["INGRESS_TRAFFIC_ALL", "INGRESS_TRAFFIC_INTERNAL_ONLY", "INGRESS_TRAFFIC_INTERNAL_LOAD_BALANCER"]</rdfs:comment>
    <rdfs:domain rdf:resource="http://example.org/onto/class/google_cloud_run_v2_service"/>
    <rdfs:range rdf:resource="http://www.w3.org/2001/XMLSchema#string"/>
  </owl:DatatypeProperty>
  <owl:DatatypeProperty rdf:about="http://example.org/onto/prop/google_cloud_run_v2_service_invoker_iam_disabled">
    <rdfs:label>invoker_iam_disabled</rdfs:label>
    <rdfs:comment>Disables IAM permission check for run.routes.invoke for callers of this service. For more information, visit https://cloud.google.com/run/docs/securing/managing-access#invoker_check.</rdfs:comment>
    <rdfs:domain rdf:resource="http://example.org/onto/class/google_cloud_run_v2_service"/>
    <rdfs:range rdf:resource="http://www.w3.org/2001/XMLSchema#string"/>
  </owl:DatatypeProperty>
  <owl:DatatypeProperty rdf:about="http://example.org/onto/prop/google_cloud_run_v2_service_labels">
    <rdfs:label>labels</rdfs:label>
    <rdfs:comment>Unstructured key value map that can be used to organize and categorize objects. User-provided labels are shared with Google's billing system, so they can be used to filter, or break down billing charges by team, component,
environment, state, etc. For more information, visit https://cloud.google.com/resource-manager/docs/creating-managing-labels or https://cloud.google.com/run/docs/configuring/labels.

Cloud Run API v2 does not support labels with  'run.googleapis.com', 'cloud.googleapis.com', 'serving.knative.dev', or 'autoscaling.knative.dev' namespaces, and they will be rejected.
All system labels in v1 now have a corresponding field in v2 Service.

**Note**: This field is non-authoritative, and will only manage the labels present in your configuration.
Please refer to the field 'effective_labels' for all of the labels present on the resource.</rdfs:comment>
    <rdfs:domain rdf:resource="http://example.org/onto/class/google_cloud_run_v2_service"/>
    <rdfs:range rdf:resource="http://www.w3.org/2001/XMLSchema#string"/>
  </owl:DatatypeProperty>
  <owl:DatatypeProperty rdf:about="http://example.org/onto/prop/google_cloud_run_v2_service_last_modifier">
    <rdfs:label>last_modifier</rdfs:label>
    <rdfs:comment>Email address of the last authenticated modifier.</rdfs:comment>
    <rdfs:domain rdf:resource="http://example.org/onto/class/google_cloud_run_v2_service"/>
    <rdfs:range rdf:resource="http://www.w3.org/2001/XMLSchema#string"/>
  </owl:DatatypeProperty>
  <owl:DatatypeProperty rdf:about="http://example.org/onto/prop/google_cloud_run_v2_service_latest_created_revision">
    <rdfs:label>latest_created_revision</rdfs:label>
    <rdfs:comment>Name of the last created revision. See comments in reconciling for additional information on reconciliation process in Cloud Run.</rdfs:comment>
    <rdfs:domain rdf:resource="http://example.org/onto/class/google_cloud_run_v2_service"/>
    <rdfs:range rdf:resource="http://www.w3.org/2001/XMLSchema#string"/>
  </owl:DatatypeProperty>
  <owl:DatatypeProperty rdf:about="http://example.org/onto/prop/google_cloud_run_v2_service_latest_ready_revision">
    <rdfs:label>latest_ready_revision</rdfs:label>
    <rdfs:comment>Name of the latest revision that is serving traffic. See comments in reconciling for additional information on reconciliation process in Cloud Run.</rdfs:comment>
    <rdfs:domain rdf:resource="http://example.org/onto/class/google_cloud_run_v2_service"/>
    <rdfs:range rdf:resource="http://www.w3.org/2001/XMLSchema#string"/>
  </owl:DatatypeProperty>
  <owl:DatatypeProperty rdf:about="http://example.org/onto/prop/google_cloud_run_v2_service_launch_stage">
    <rdfs:label>launch_stage</rdfs:label>
    <rdfs:comment>The launch stage as defined by [Google Cloud Platform Launch Stages](https://cloud.google.com/products#product-launch-stages). Cloud Run supports ALPHA, BETA, and GA.
If no value is specified, GA is assumed. Set the launch stage to a preview stage on input to allow use of preview features in that stage. On read (or output), describes whether the resource uses preview features.

For example, if ALPHA is provided as input, but only BETA and GA-level features are used, this field will be BETA on output. Possible values: ["UNIMPLEMENTED", "PRELAUNCH", "EARLY_ACCESS", "ALPHA", "BETA", "GA", "DEPRECATED"]</rdfs:comment>
    <rdfs:domain rdf:resource="http://example.org/onto/class/google_cloud_run_v2_service"/>
    <rdfs:range rdf:resource="http://www.w3.org/2001/XMLSchema#string"/>
  </owl:DatatypeProperty>
  <owl:DatatypeProperty rdf:about="http://example.org/onto/prop/google_cloud_run_v2_service_location">
    <rdfs:label>location</rdfs:label>
    <rdfs:comment>The location of the cloud run service</rdfs:comment>
    <rdfs:domain rdf:resource="http://example.org/onto/class/google_cloud_run_v2_service"/>
    <rdfs:range rdf:resource="http://www.w3.org/2001/XMLSchema#string"/>
  </owl:DatatypeProperty>
  <owl:DatatypeProperty rdf:about="http://example.org/onto/prop/google_cloud_run_v2_service_name">
    <rdfs:label>name</rdfs:label>
    <rdfs:comment>Name of the Service.</rdfs:comment>
    <rdfs:domain rdf:resource="http://example.org/onto/class/google_cloud_run_v2_service"/>
    <rdfs:range rdf:resource="http://www.w3.org/2001/XMLSchema#string"/>
  </owl:DatatypeProperty>
  <owl:DatatypeProperty rdf:about="http://example.org/onto/prop/google_cloud_run_v2_service_observed_generation">
    <rdfs:label>observed_generation</rdfs:label>
    <rdfs:comment>The generation of this Service currently serving traffic. See comments in reconciling for additional information on reconciliation process in Cloud Run. Please note that unlike v1, this is an int64 value. As with most Google APIs, its JSON representation will be a string instead of an integer.</rdfs:comment>
    <rdfs:domain rdf:resource="http://example.org/onto/class/google_cloud_run_v2_service"/>
    <rdfs:range rdf:resource="http://www.w3.org/2001/XMLSchema#string"/>
  </owl:DatatypeProperty>
  <owl:DatatypeProperty rdf:about="http://example.org/onto/prop/google_cloud_run_v2_service_project">
    <rdfs:label>project</rdfs:label>
    <rdfs:domain rdf:resource="http://example.org/onto/class/google_cloud_run_v2_service"/>
    <rdfs:range rdf:resource="http://www.w3.org/2001/XMLSchema#string"/>
  </owl:DatatypeProperty>
  <owl:DatatypeProperty rdf:about="http://example.org/onto/prop/google_cloud_run_v2_service_reconciling">
    <rdfs:label>reconciling</rdfs:label>
    <rdfs:comment>Returns true if the Service is currently being acted upon by the system to bring it into the desired state.

When a new Service is created, or an existing one is updated, Cloud Run will asynchronously perform all necessary steps to bring the Service to the desired serving state. This process is called reconciliation. While reconciliation is in process, observedGeneration, latest_ready_revison, trafficStatuses, and uri will have transient values that might mismatch the intended state: Once reconciliation is over (and this field is false), there are two possible outcomes: reconciliation succeeded and the serving state matches the Service, or there was an error, and reconciliation failed. This state can be found in terminalCondition.state.

If reconciliation succeeded, the following fields will match: traffic and trafficStatuses, observedGeneration and generation, latestReadyRevision and latestCreatedRevision.

If reconciliation failed, trafficStatuses, observedGeneration, and latestReadyRevision will have the state of the last serving revision, or empty for newly created Services. Additional information on the failure can be found in terminalCondition and conditions.</rdfs:comment>
    <rdfs:domain rdf:resource="http://example.org/onto/class/google_cloud_run_v2_service"/>
    <rdfs:range rdf:resource="http://www.w3.org/2001/XMLSchema#string"/>
  </owl:DatatypeProperty>
  <owl:DatatypeProperty rdf:about="http://example.org/onto/prop/google_cloud_run_v2_service_terminal_condition">
    <rdfs:label>terminal_condition</rdfs:label>
    <rdfs:comment>The Condition of this Service, containing its readiness status, and detailed error information in case it did not reach a serving state. See comments in reconciling for additional information on reconciliation process in Cloud Run.</rdfs:comment>
    <rdfs:domain rdf:resource="http://example.org/onto/class/google_cloud_run_v2_service"/>
    <rdfs:range rdf:resource="http://www.w3.org/2001/XMLSchema#string"/>
  </owl:DatatypeProperty>
  <owl:DatatypeProperty rdf:about="http://example.org/onto/prop/google_cloud_run_v2_service_terraform_labels">
    <rdfs:label>terraform_labels</rdfs:label>
    <rdfs:comment>The combination of labels configured directly on the resource
 and default labels configured on the provider.</rdfs:comment>
    <rdfs:domain rdf:resource="http://example.org/onto/class/google_cloud_run_v2_service"/>
    <rdfs:range rdf:resource="http://www.w3.org/2001/XMLSchema#string"/>
  </owl:DatatypeProperty>
  <owl:DatatypeProperty rdf:about="http://example.org/onto/prop/google_cloud_run_v2_service_traffic_statuses">
    <rdfs:label>traffic_statuses</rdfs:label>
    <rdfs:comment>Detailed status information for corresponding traffic targets. See comments in reconciling for additional information on reconciliation process in Cloud Run.</rdfs:comment>
    <rdfs:domain rdf:resource="http://example.org/onto/class/google_cloud_run_v2_service"/>
    <rdfs:range rdf:resource="http://www.w3.org/2001/XMLSchema#string"/>
  </owl:DatatypeProperty>
  <owl:DatatypeProperty rdf:about="http://example.org/onto/prop/google_cloud_run_v2_service_uid">
    <rdfs:label>uid</rdfs:label>
    <rdfs:comment>Server assigned unique identifier for the trigger. The value is a UUID4 string and guaranteed to remain unchanged until the resource is deleted.</rdfs:comment>
    <rdfs:domain rdf:resource="http://example.org/onto/class/google_cloud_run_v2_service"/>
    <rdfs:range rdf:resource="http://www.w3.org/2001/XMLSchema#string"/>
  </owl:DatatypeProperty>
  <owl:DatatypeProperty rdf:about="http://example.org/onto/prop/google_cloud_run_v2_service_update_time">
    <rdfs:label>update_time</rdfs:label>
    <rdfs:comment>The last-modified time.</rdfs:comment>
    <rdfs:domain rdf:resource="http://example.org/onto/class/google_cloud_run_v2_service"/>
    <rdfs:range rdf:resource="http://www.w3.org/2001/XMLSchema#string"/>
  </owl:DatatypeProperty>
  <owl:DatatypeProperty rdf:about="http://example.org/onto/prop/google_cloud_run_v2_service_uri">
    <rdfs:label>uri</rdfs:label>
    <rdfs:comment>The main URI in which this Service is serving traffic.</rdfs:comment>
    <rdfs:domain rdf:resource="http://example.org/onto/class/google_cloud_run_v2_service"/>
    <rdfs:range rdf:resource="http://www.w3.org/2001/XMLSchema#string"/>
  </owl:DatatypeProperty>
  <owl:DatatypeProperty rdf:about="http://example.org/onto/prop/google_cloud_run_v2_service_urls">
    <rdfs:label>urls</rdfs:label>
    <rdfs:comment>All URLs serving traffic for this Service.</rdfs:comment>
    <rdfs:domain rdf:resource="http://example.org/onto/class/google_cloud_run_v2_service"/>
    <rdfs:range rdf:resource="http://www.w3.org/2001/XMLSchema#string"/>
  </owl:DatatypeProperty>
  <owl:DatatypeProperty rdf:about="http://example.org/onto/prop/google_cloud_run_v2_service_breakglass_justification">
    <rdfs:label>breakglass_justification</rdfs:label>
    <rdfs:comment>If present, indicates to use Breakglass using this justification. If useDefault is False, then it must be empty. For more information on breakglass, see https://cloud.google.com/binary-authorization/docs/using-breakglass</rdfs:comment>
    <rdfs:domain rdf:resource="http://example.org/onto/class/google_cloud_run_v2_service"/>
    <rdfs:range rdf:resource="http://www.w3.org/2001/XMLSchema#string"/>
  </owl:DatatypeProperty>
  <owl:DatatypeProperty rdf:about="http://example.org/onto/prop/google_cloud_run_v2_service_policy">
    <rdfs:label>policy</rdfs:label>
    <rdfs:comment>The path to a binary authorization policy. Format: projects/{project}/platforms/cloudRun/{policy-name}</rdfs:comment>
    <rdfs:domain rdf:resource="http://example.org/onto/class/google_cloud_run_v2_service"/>
    <rdfs:range rdf:resource="http://www.w3.org/2001/XMLSchema#string"/>
  </owl:DatatypeProperty>
  <owl:DatatypeProperty rdf:about="http://example.org/onto/prop/google_cloud_run_v2_service_use_default">
    <rdfs:label>use_default</rdfs:label>
    <rdfs:comment>If True, indicates to use the default project's binary authorization policy. If False, binary authorization will be disabled.</rdfs:comment>
    <rdfs:domain rdf:resource="http://example.org/onto/class/google_cloud_run_v2_service"/>
    <rdfs:range rdf:resource="http://www.w3.org/2001/XMLSchema#string"/>
  </owl:DatatypeProperty>
  <owl:DatatypeProperty rdf:about="http://example.org/onto/prop/google_cloud_run_v2_service_base_image">
    <rdfs:label>base_image</rdfs:label>
    <rdfs:comment>The base image used to build the function.</rdfs:comment>
    <rdfs:domain rdf:resource="http://example.org/onto/class/google_cloud_run_v2_service"/>
    <rdfs:range rdf:resource="http://www.w3.org/2001/XMLSchema#string"/>
  </owl:DatatypeProperty>
  <owl:DatatypeProperty rdf:about="http://example.org/onto/prop/google_cloud_run_v2_service_enable_automatic_updates">
    <rdfs:label>enable_automatic_updates</rdfs:label>
    <rdfs:comment>Sets whether the function will receive automatic base image updates.</rdfs:comment>
    <rdfs:domain rdf:resource="http://example.org/onto/class/google_cloud_run_v2_service"/>
    <rdfs:range rdf:resource="http://www.w3.org/2001/XMLSchema#string"/>
  </owl:DatatypeProperty>
  <owl:DatatypeProperty rdf:about="http://example.org/onto/prop/google_cloud_run_v2_service_environment_variables">
    <rdfs:label>environment_variables</rdfs:label>
    <rdfs:comment>User-provided build-time environment variables for the function.</rdfs:comment>
    <rdfs:domain rdf:resource="http://example.org/onto/class/google_cloud_run_v2_service"/>
    <rdfs:range rdf:resource="http://www.w3.org/2001/XMLSchema#string"/>
  </owl:DatatypeProperty>
  <owl:DatatypeProperty rdf:about="http://example.org/onto/prop/google_cloud_run_v2_service_function_target">
    <rdfs:label>function_target</rdfs:label>
    <rdfs:comment>The name of the function (as defined in source code) that will be executed. Defaults to the resource name suffix, if not specified. For backward compatibility, if function with given name is not found, then the system will try to use function named "function".</rdfs:comment>
    <rdfs:domain rdf:resource="http://example.org/onto/class/google_cloud_run_v2_service"/>
    <rdfs:range rdf:resource="http://www.w3.org/2001/XMLSchema#string"/>
  </owl:DatatypeProperty>
  <owl:DatatypeProperty rdf:about="http://example.org/onto/prop/google_cloud_run_v2_service_image_uri">
    <rdfs:label>image_uri</rdfs:label>
    <rdfs:comment>Artifact Registry URI to store the built image.</rdfs:comment>
    <rdfs:domain rdf:resource="http://example.org/onto/class/google_cloud_run_v2_service"/>
    <rdfs:range rdf:resource="http://www.w3.org/2001/XMLSchema#string"/>
  </owl:DatatypeProperty>
  <owl:DatatypeProperty rdf:about="http://example.org/onto/prop/google_cloud_run_v2_service_name">
    <rdfs:label>name</rdfs:label>
    <rdfs:comment>The Cloud Build name of the latest successful deployment of the function.</rdfs:comment>
    <rdfs:domain rdf:resource="http://example.org/onto/class/google_cloud_run_v2_service"/>
    <rdfs:range rdf:resource="http://www.w3.org/2001/XMLSchema#string"/>
  </owl:DatatypeProperty>
  <owl:DatatypeProperty rdf:about="http://example.org/onto/prop/google_cloud_run_v2_service_service_account">
    <rdfs:label>service_account</rdfs:label>
    <rdfs:comment>Service account to be used for building the container. The format of this field is 'projects/{projectId}/serviceAccounts/{serviceAccountEmail}'.</rdfs:comment>
    <rdfs:domain rdf:resource="http://example.org/onto/class/google_cloud_run_v2_service"/>
    <rdfs:range rdf:resource="http://www.w3.org/2001/XMLSchema#string"/>
  </owl:DatatypeProperty>
  <owl:DatatypeProperty rdf:about="http://example.org/onto/prop/google_cloud_run_v2_service_source_location">
    <rdfs:label>source_location</rdfs:label>
    <rdfs:comment>The Cloud Storage bucket URI where the function source code is located.</rdfs:comment>
    <rdfs:domain rdf:resource="http://example.org/onto/class/google_cloud_run_v2_service"/>
    <rdfs:range rdf:resource="http://www.w3.org/2001/XMLSchema#string"/>
  </owl:DatatypeProperty>
  <owl:DatatypeProperty rdf:about="http://example.org/onto/prop/google_cloud_run_v2_service_worker_pool">
    <rdfs:label>worker_pool</rdfs:label>
    <rdfs:comment>Name of the Cloud Build Custom Worker Pool that should be used to build the Cloud Run function. The format of this field is 'projects/{project}/locations/{region}/workerPools/{workerPool}' where {project} and {region} are the project id and region respectively where the worker pool is defined and {workerPool} is the short name of the worker pool.</rdfs:comment>
    <rdfs:domain rdf:resource="http://example.org/onto/class/google_cloud_run_v2_service"/>
    <rdfs:range rdf:resource="http://www.w3.org/2001/XMLSchema#string"/>
  </owl:DatatypeProperty>
  <owl:DatatypeProperty rdf:about="http://example.org/onto/prop/google_cloud_run_v2_service_multi_region_id">
    <rdfs:label>multi_region_id</rdfs:label>
    <rdfs:comment>System-generated unique id for the multi-region Service.</rdfs:comment>
    <rdfs:domain rdf:resource="http://example.org/onto/class/google_cloud_run_v2_service"/>
    <rdfs:range rdf:resource="http://www.w3.org/2001/XMLSchema#string"/>
  </owl:DatatypeProperty>
  <owl:DatatypeProperty rdf:about="http://example.org/onto/prop/google_cloud_run_v2_service_regions">
    <rdfs:label>regions</rdfs:label>
    <rdfs:comment>The list of regions to deploy the multi-region Service.</rdfs:comment>
    <rdfs:domain rdf:resource="http://example.org/onto/class/google_cloud_run_v2_service"/>
    <rdfs:range rdf:resource="http://www.w3.org/2001/XMLSchema#string"/>
  </owl:DatatypeProperty>
  <owl:DatatypeProperty rdf:about="http://example.org/onto/prop/google_cloud_run_v2_service_manual_instance_count">
    <rdfs:label>manual_instance_count</rdfs:label>
    <rdfs:comment>Total instance count for the service in manual scaling mode. This number of instances is divided among all revisions with specified traffic based on the percent of traffic they are receiving.</rdfs:comment>
    <rdfs:domain rdf:resource="http://example.org/onto/class/google_cloud_run_v2_service"/>
    <rdfs:range rdf:resource="http://www.w3.org/2001/XMLSchema#string"/>
  </owl:DatatypeProperty>
  <owl:DatatypeProperty rdf:about="http://example.org/onto/prop/google_cloud_run_v2_service_max_instance_count">
    <rdfs:label>max_instance_count</rdfs:label>
    <rdfs:comment>Combined maximum number of instances for all revisions receiving traffic.</rdfs:comment>
    <rdfs:domain rdf:resource="http://example.org/onto/class/google_cloud_run_v2_service"/>
    <rdfs:range rdf:resource="http://www.w3.org/2001/XMLSchema#string"/>
  </owl:DatatypeProperty>
  <owl:DatatypeProperty rdf:about="http://example.org/onto/prop/google_cloud_run_v2_service_min_instance_count">
    <rdfs:label>min_instance_count</rdfs:label>
    <rdfs:comment>Minimum number of instances for the service, to be divided among all revisions receiving traffic.</rdfs:comment>
    <rdfs:domain rdf:resource="http://example.org/onto/class/google_cloud_run_v2_service"/>
    <rdfs:range rdf:resource="http://www.w3.org/2001/XMLSchema#string"/>
  </owl:DatatypeProperty>
  <owl:DatatypeProperty rdf:about="http://example.org/onto/prop/google_cloud_run_v2_service_scaling_mode">
    <rdfs:label>scaling_mode</rdfs:label>
    <rdfs:comment>The [scaling mode](https://cloud.google.com/run/docs/reference/rest/v2/projects.locations.services#scalingmode) for the service. Possible values: ["AUTOMATIC", "MANUAL"]</rdfs:comment>
    <rdfs:domain rdf:resource="http://example.org/onto/class/google_cloud_run_v2_service"/>
    <rdfs:range rdf:resource="http://www.w3.org/2001/XMLSchema#string"/>
  </owl:DatatypeProperty>
  <owl:DatatypeProperty rdf:about="http://example.org/onto/prop/google_cloud_run_v2_service_annotations">
    <rdfs:label>annotations</rdfs:label>
    <rdfs:comment>Unstructured key value map that may be set by external tools to store and arbitrary metadata. They are not queryable and should be preserved when modifying objects.

Cloud Run API v2 does not support annotations with 'run.googleapis.com', 'cloud.googleapis.com', 'serving.knative.dev', or 'autoscaling.knative.dev' namespaces, and they will be rejected.
All system annotations in v1 now have a corresponding field in v2 RevisionTemplate.

This field follows Kubernetes annotations' namespacing, limits, and rules.</rdfs:comment>
    <rdfs:domain rdf:resource="http://example.org/onto/class/google_cloud_run_v2_service"/>
    <rdfs:range rdf:resource="http://www.w3.org/2001/XMLSchema#string"/>
  </owl:DatatypeProperty>
  <owl:DatatypeProperty rdf:about="http://example.org/onto/prop/google_cloud_run_v2_service_encryption_key">
    <rdfs:label>encryption_key</rdfs:label>
    <rdfs:comment>A reference to a customer managed encryption key (CMEK) to use to encrypt this container image. For more information, go to https://cloud.google.com/run/docs/securing/using-cmek</rdfs:comment>
    <rdfs:domain rdf:resource="http://example.org/onto/class/google_cloud_run_v2_service"/>
    <rdfs:range rdf:resource="http://www.w3.org/2001/XMLSchema#string"/>
  </owl:DatatypeProperty>
  <owl:DatatypeProperty rdf:about="http://example.org/onto/prop/google_cloud_run_v2_service_execution_environment">
    <rdfs:label>execution_environment</rdfs:label>
    <rdfs:comment>The sandbox environment to host this Revision. Possible values: ["EXECUTION_ENVIRONMENT_GEN1", "EXECUTION_ENVIRONMENT_GEN2"]</rdfs:comment>
    <rdfs:domain rdf:resource="http://example.org/onto/class/google_cloud_run_v2_service"/>
    <rdfs:range rdf:resource="http://www.w3.org/2001/XMLSchema#string"/>
  </owl:DatatypeProperty>
  <owl:DatatypeProperty rdf:about="http://example.org/onto/prop/google_cloud_run_v2_service_gpu_zonal_redundancy_disabled">
    <rdfs:label>gpu_zonal_redundancy_disabled</rdfs:label>
    <rdfs:comment>True if GPU zonal redundancy is disabled on this revision.</rdfs:comment>
    <rdfs:domain rdf:resource="http://example.org/onto/class/google_cloud_run_v2_service"/>
    <rdfs:range rdf:resource="http://www.w3.org/2001/XMLSchema#string"/>
  </owl:DatatypeProperty>
  <owl:DatatypeProperty rdf:about="http://example.org/onto/prop/google_cloud_run_v2_service_health_check_disabled">
    <rdfs:label>health_check_disabled</rdfs:label>
    <rdfs:comment>Disables health checking containers during deployment.</rdfs:comment>
    <rdfs:domain rdf:resource="http://example.org/onto/class/google_cloud_run_v2_service"/>
    <rdfs:range rdf:resource="http://www.w3.org/2001/XMLSchema#string"/>
  </owl:DatatypeProperty>
  <owl:DatatypeProperty rdf:about="http://example.org/onto/prop/google_cloud_run_v2_service_labels">
    <rdfs:label>labels</rdfs:label>
    <rdfs:comment>Unstructured key value map that can be used to organize and categorize objects. User-provided labels are shared with Google's billing system, so they can be used to filter, or break down billing charges by team, component, environment, state, etc.
For more information, visit https://cloud.google.com/resource-manager/docs/creating-managing-labels or https://cloud.google.com/run/docs/configuring/labels.

Cloud Run API v2 does not support labels with 'run.googleapis.com', 'cloud.googleapis.com', 'serving.knative.dev', or 'autoscaling.knative.dev' namespaces, and they will be rejected.
All system labels in v1 now have a corresponding field in v2 RevisionTemplate.</rdfs:comment>
    <rdfs:domain rdf:resource="http://example.org/onto/class/google_cloud_run_v2_service"/>
    <rdfs:range rdf:resource="http://www.w3.org/2001/XMLSchema#string"/>
  </owl:DatatypeProperty>
  <owl:DatatypeProperty rdf:about="http://example.org/onto/prop/google_cloud_run_v2_service_max_instance_request_concurrency">
    <rdfs:label>max_instance_request_concurrency</rdfs:label>
    <rdfs:comment>Sets the maximum number of requests that each serving instance can receive.
If not specified or 0, defaults to 80 when requested CPU >= 1 and defaults to 1 when requested CPU < 1.</rdfs:comment>
    <rdfs:domain rdf:resource="http://example.org/onto/class/google_cloud_run_v2_service"/>
    <rdfs:range rdf:resource="http://www.w3.org/2001/XMLSchema#string"/>
  </owl:DatatypeProperty>
  <owl:DatatypeProperty rdf:about="http://example.org/onto/prop/google_cloud_run_v2_service_revision">
    <rdfs:label>revision</rdfs:label>
    <rdfs:comment>The unique name for the revision. If this field is omitted, it will be automatically generated based on the Service name.</rdfs:comment>
    <rdfs:domain rdf:resource="http://example.org/onto/class/google_cloud_run_v2_service"/>
    <rdfs:range rdf:resource="http://www.w3.org/2001/XMLSchema#string"/>
  </owl:DatatypeProperty>
  <owl:DatatypeProperty rdf:about="http://example.org/onto/prop/google_cloud_run_v2_service_service_account">
    <rdfs:label>service_account</rdfs:label>
    <rdfs:comment>Email address of the IAM service account associated with the revision of the service. The service account represents the identity of the running revision, and determines what permissions the revision has. If not provided, the revision will use the project's default service account.</rdfs:comment>
    <rdfs:domain rdf:resource="http://example.org/onto/class/google_cloud_run_v2_service"/>
    <rdfs:range rdf:resource="http://www.w3.org/2001/XMLSchema#string"/>
  </owl:DatatypeProperty>
  <owl:DatatypeProperty rdf:about="http://example.org/onto/prop/google_cloud_run_v2_service_session_affinity">
    <rdfs:label>session_affinity</rdfs:label>
    <rdfs:comment>Enables session affinity. For more information, go to https://cloud.google.com/run/docs/configuring/session-affinity</rdfs:comment>
    <rdfs:domain rdf:resource="http://example.org/onto/class/google_cloud_run_v2_service"/>
    <rdfs:range rdf:resource="http://www.w3.org/2001/XMLSchema#string"/>
  </owl:DatatypeProperty>
  <owl:DatatypeProperty rdf:about="http://example.org/onto/prop/google_cloud_run_v2_service_timeout">
    <rdfs:label>timeout</rdfs:label>
    <rdfs:comment>Max allowed time for an instance to respond to a request.

A duration in seconds with up to nine fractional digits, ending with 's'. Example: "3.5s".</rdfs:comment>
    <rdfs:domain rdf:resource="http://example.org/onto/class/google_cloud_run_v2_service"/>
    <rdfs:range rdf:resource="http://www.w3.org/2001/XMLSchema#string"/>
  </owl:DatatypeProperty>
  <owl:DatatypeProperty rdf:about="http://example.org/onto/prop/google_cloud_run_v2_service_args">
    <rdfs:label>args</rdfs:label>
    <rdfs:comment>Arguments to the entrypoint. The docker image's CMD is used if this is not provided. Variable references are not supported in Cloud Run.</rdfs:comment>
    <rdfs:domain rdf:resource="http://example.org/onto/class/google_cloud_run_v2_service"/>
    <rdfs:range rdf:resource="http://www.w3.org/2001/XMLSchema#string"/>
  </owl:DatatypeProperty>
  <owl:DatatypeProperty rdf:about="http://example.org/onto/prop/google_cloud_run_v2_service_base_image_uri">
    <rdfs:label>base_image_uri</rdfs:label>
    <rdfs:comment>Base image for this container. If set, it indicates that the service is enrolled into automatic base image update.</rdfs:comment>
    <rdfs:domain rdf:resource="http://example.org/onto/class/google_cloud_run_v2_service"/>
    <rdfs:range rdf:resource="http://www.w3.org/2001/XMLSchema#string"/>
  </owl:DatatypeProperty>
  <owl:DatatypeProperty rdf:about="http://example.org/onto/prop/google_cloud_run_v2_service_build_info">
    <rdfs:label>build_info</rdfs:label>
    <rdfs:comment>The build info of the container image.</rdfs:comment>
    <rdfs:domain rdf:resource="http://example.org/onto/class/google_cloud_run_v2_service"/>
    <rdfs:range rdf:resource="http://www.w3.org/2001/XMLSchema#string"/>
  </owl:DatatypeProperty>
  <owl:DatatypeProperty rdf:about="http://example.org/onto/prop/google_cloud_run_v2_service_command">
    <rdfs:label>command</rdfs:label>
    <rdfs:comment>Entrypoint array. Not executed within a shell. The docker image's ENTRYPOINT is used if this is not provided. Variable references $(VAR_NAME) are expanded using the container's environment. If a variable cannot be resolved, the reference in the input string will be unchanged. The $(VAR_NAME) syntax can be escaped with a double $$, ie: $$(VAR_NAME). Escaped references will never be expanded, regardless of whether the variable exists or not. More info: https://kubernetes.io/docs/tasks/inject-data-application/define-command-argument-container/#running-a-command-in-a-shell</rdfs:comment>
    <rdfs:domain rdf:resource="http://example.org/onto/class/google_cloud_run_v2_service"/>
    <rdfs:range rdf:resource="http://www.w3.org/2001/XMLSchema#string"/>
  </owl:DatatypeProperty>
  <owl:DatatypeProperty rdf:about="http://example.org/onto/prop/google_cloud_run_v2_service_depends_on">
    <rdfs:label>depends_on</rdfs:label>
    <rdfs:comment>Containers which should be started before this container. If specified the container will wait to start until all containers with the listed names are healthy.</rdfs:comment>
    <rdfs:domain rdf:resource="http://example.org/onto/class/google_cloud_run_v2_service"/>
    <rdfs:range rdf:resource="http://www.w3.org/2001/XMLSchema#string"/>
  </owl:DatatypeProperty>
  <owl:DatatypeProperty rdf:about="http://example.org/onto/prop/google_cloud_run_v2_service_image">
    <rdfs:label>image</rdfs:label>
    <rdfs:comment>URL of the Container image in Google Container Registry or Google Artifact Registry. More info: https://kubernetes.io/docs/concepts/containers/images</rdfs:comment>
    <rdfs:domain rdf:resource="http://example.org/onto/class/google_cloud_run_v2_service"/>
    <rdfs:range rdf:resource="http://www.w3.org/2001/XMLSchema#string"/>
  </owl:DatatypeProperty>
  <owl:DatatypeProperty rdf:about="http://example.org/onto/prop/google_cloud_run_v2_service_name">
    <rdfs:label>name</rdfs:label>
    <rdfs:comment>Name of the container specified as a DNS_LABEL.</rdfs:comment>
    <rdfs:domain rdf:resource="http://example.org/onto/class/google_cloud_run_v2_service"/>
    <rdfs:range rdf:resource="http://www.w3.org/2001/XMLSchema#string"/>
  </owl:DatatypeProperty>
  <owl:DatatypeProperty rdf:about="http://example.org/onto/prop/google_cloud_run_v2_service_working_dir">
    <rdfs:label>working_dir</rdfs:label>
    <rdfs:comment>Container's working directory. If not specified, the container runtime's default will be used, which might be configured in the container image.</rdfs:comment>
    <rdfs:domain rdf:resource="http://example.org/onto/class/google_cloud_run_v2_service"/>
    <rdfs:range rdf:resource="http://www.w3.org/2001/XMLSchema#string"/>
  </owl:DatatypeProperty>
  <owl:DatatypeProperty rdf:about="http://example.org/onto/prop/google_cloud_run_v2_service_name">
    <rdfs:label>name</rdfs:label>
    <rdfs:comment>Name of the environment variable. Must be a C_IDENTIFIER, and may not exceed 32768 characters.</rdfs:comment>
    <rdfs:domain rdf:resource="http://example.org/onto/class/google_cloud_run_v2_service"/>
    <rdfs:range rdf:resource="http://www.w3.org/2001/XMLSchema#string"/>
  </owl:DatatypeProperty>
  <owl:DatatypeProperty rdf:about="http://example.org/onto/prop/google_cloud_run_v2_service_value">
    <rdfs:label>value</rdfs:label>
    <rdfs:comment>Literal value of the environment variable. Defaults to "" and the maximum allowed length is 32768 characters. Variable references are not supported in Cloud Run.</rdfs:comment>
    <rdfs:domain rdf:resource="http://example.org/onto/class/google_cloud_run_v2_service"/>
    <rdfs:range rdf:resource="http://www.w3.org/2001/XMLSchema#string"/>
  </owl:DatatypeProperty>
  <owl:DatatypeProperty rdf:about="http://example.org/onto/prop/google_cloud_run_v2_service_secret">
    <rdfs:label>secret</rdfs:label>
    <rdfs:comment>The name of the secret in Cloud Secret Manager. Format: {secretName} if the secret is in the same project. projects/{project}/secrets/{secretName} if the secret is in a different project.</rdfs:comment>
    <rdfs:domain rdf:resource="http://example.org/onto/class/google_cloud_run_v2_service"/>
    <rdfs:range rdf:resource="http://www.w3.org/2001/XMLSchema#string"/>
  </owl:DatatypeProperty>
  <owl:DatatypeProperty rdf:about="http://example.org/onto/prop/google_cloud_run_v2_service_version">
    <rdfs:label>version</rdfs:label>
    <rdfs:comment>The Cloud Secret Manager secret version. Can be 'latest' for the latest value or an integer for a specific version.</rdfs:comment>
    <rdfs:domain rdf:resource="http://example.org/onto/class/google_cloud_run_v2_service"/>
    <rdfs:range rdf:resource="http://www.w3.org/2001/XMLSchema#string"/>
  </owl:DatatypeProperty>
  <owl:DatatypeProperty rdf:about="http://example.org/onto/prop/google_cloud_run_v2_service_failure_threshold">
    <rdfs:label>failure_threshold</rdfs:label>
    <rdfs:comment>Minimum consecutive failures for the probe to be considered failed after having succeeded. Defaults to 3. Minimum value is 1.</rdfs:comment>
    <rdfs:domain rdf:resource="http://example.org/onto/class/google_cloud_run_v2_service"/>
    <rdfs:range rdf:resource="http://www.w3.org/2001/XMLSchema#string"/>
  </owl:DatatypeProperty>
  <owl:DatatypeProperty rdf:about="http://example.org/onto/prop/google_cloud_run_v2_service_initial_delay_seconds">
    <rdfs:label>initial_delay_seconds</rdfs:label>
    <rdfs:comment>Number of seconds after the container has started before the probe is initiated. Defaults to 0 seconds. Minimum value is 0. Maximum value for liveness probe is 3600. Maximum value for startup probe is 240. More info: https://kubernetes.io/docs/concepts/workloads/pods/pod-lifecycle#container-probes</rdfs:comment>
    <rdfs:domain rdf:resource="http://example.org/onto/class/google_cloud_run_v2_service"/>
    <rdfs:range rdf:resource="http://www.w3.org/2001/XMLSchema#string"/>
  </owl:DatatypeProperty>
  <owl:DatatypeProperty rdf:about="http://example.org/onto/prop/google_cloud_run_v2_service_period_seconds">
    <rdfs:label>period_seconds</rdfs:label>
    <rdfs:comment>How often (in seconds) to perform the probe. Default to 10 seconds. Minimum value is 1. Maximum value for liveness probe is 3600. Maximum value for startup probe is 240. Must be greater or equal than timeoutSeconds</rdfs:comment>
    <rdfs:domain rdf:resource="http://example.org/onto/class/google_cloud_run_v2_service"/>
    <rdfs:range rdf:resource="http://www.w3.org/2001/XMLSchema#string"/>
  </owl:DatatypeProperty>
  <owl:DatatypeProperty rdf:about="http://example.org/onto/prop/google_cloud_run_v2_service_timeout_seconds">
    <rdfs:label>timeout_seconds</rdfs:label>
    <rdfs:comment>Number of seconds after which the probe times out. Defaults to 1 second. Minimum value is 1. Maximum value is 3600. Must be smaller than periodSeconds. More info: https://kubernetes.io/docs/concepts/workloads/pods/pod-lifecycle#container-probes</rdfs:comment>
    <rdfs:domain rdf:resource="http://example.org/onto/class/google_cloud_run_v2_service"/>
    <rdfs:range rdf:resource="http://www.w3.org/2001/XMLSchema#string"/>
  </owl:DatatypeProperty>
  <owl:DatatypeProperty rdf:about="http://example.org/onto/prop/google_cloud_run_v2_service_port">
    <rdfs:label>port</rdfs:label>
    <rdfs:comment>Port number to access on the container. Number must be in the range 1 to 65535.
If not specified, defaults to the same value as container.ports[0].containerPort.</rdfs:comment>
    <rdfs:domain rdf:resource="http://example.org/onto/class/google_cloud_run_v2_service"/>
    <rdfs:range rdf:resource="http://www.w3.org/2001/XMLSchema#string"/>
  </owl:DatatypeProperty>
  <owl:DatatypeProperty rdf:about="http://example.org/onto/prop/google_cloud_run_v2_service_service">
    <rdfs:label>service</rdfs:label>
    <rdfs:comment>The name of the service to place in the gRPC HealthCheckRequest
(see https://github.com/grpc/grpc/blob/master/doc/health-checking.md).
If this is not specified, the default behavior is defined by gRPC.</rdfs:comment>
    <rdfs:domain rdf:resource="http://example.org/onto/class/google_cloud_run_v2_service"/>
    <rdfs:range rdf:resource="http://www.w3.org/2001/XMLSchema#string"/>
  </owl:DatatypeProperty>
  <owl:DatatypeProperty rdf:about="http://example.org/onto/prop/google_cloud_run_v2_service_path">
    <rdfs:label>path</rdfs:label>
    <rdfs:comment>Path to access on the HTTP server. Defaults to '/'.</rdfs:comment>
    <rdfs:domain rdf:resource="http://example.org/onto/class/google_cloud_run_v2_service"/>
    <rdfs:range rdf:resource="http://www.w3.org/2001/XMLSchema#string"/>
  </owl:DatatypeProperty>
  <owl:DatatypeProperty rdf:about="http://example.org/onto/prop/google_cloud_run_v2_service_port">
    <rdfs:label>port</rdfs:label>
    <rdfs:comment>Port number to access on the container. Number must be in the range 1 to 65535.
If not specified, defaults to the same value as container.ports[0].containerPort.</rdfs:comment>
    <rdfs:domain rdf:resource="http://example.org/onto/class/google_cloud_run_v2_service"/>
    <rdfs:range rdf:resource="http://www.w3.org/2001/XMLSchema#string"/>
  </owl:DatatypeProperty>
  <owl:DatatypeProperty rdf:about="http://example.org/onto/prop/google_cloud_run_v2_service_name">
    <rdfs:label>name</rdfs:label>
    <rdfs:comment>The header field name</rdfs:comment>
    <rdfs:domain rdf:resource="http://example.org/onto/class/google_cloud_run_v2_service"/>
    <rdfs:range rdf:resource="http://www.w3.org/2001/XMLSchema#string"/>
  </owl:DatatypeProperty>
  <owl:DatatypeProperty rdf:about="http://example.org/onto/prop/google_cloud_run_v2_service_value">
    <rdfs:label>value</rdfs:label>
    <rdfs:comment>The header field value</rdfs:comment>
    <rdfs:domain rdf:resource="http://example.org/onto/class/google_cloud_run_v2_service"/>
    <rdfs:range rdf:resource="http://www.w3.org/2001/XMLSchema#string"/>
  </owl:DatatypeProperty>
  <owl:DatatypeProperty rdf:about="http://example.org/onto/prop/google_cloud_run_v2_service_port">
    <rdfs:label>port</rdfs:label>
    <rdfs:comment>Port number to access on the container. Must be in the range 1 to 65535.
If not specified, defaults to the exposed port of the container, which
is the value of container.ports[0].containerPort.</rdfs:comment>
    <rdfs:domain rdf:resource="http://example.org/onto/class/google_cloud_run_v2_service"/>
    <rdfs:range rdf:resource="http://www.w3.org/2001/XMLSchema#string"/>
  </owl:DatatypeProperty>
  <owl:DatatypeProperty rdf:about="http://example.org/onto/prop/google_cloud_run_v2_service_container_port">
    <rdfs:label>container_port</rdfs:label>
    <rdfs:comment>Port number the container listens on. This must be a valid TCP port number, 0 < containerPort < 65536.</rdfs:comment>
    <rdfs:domain rdf:resource="http://example.org/onto/class/google_cloud_run_v2_service"/>
    <rdfs:range rdf:resource="http://www.w3.org/2001/XMLSchema#string"/>
  </owl:DatatypeProperty>
  <owl:DatatypeProperty rdf:about="http://example.org/onto/prop/google_cloud_run_v2_service_name">
    <rdfs:label>name</rdfs:label>
    <rdfs:comment>If specified, used to specify which protocol to use. Allowed values are "http1" and "h2c".</rdfs:comment>
    <rdfs:domain rdf:resource="http://example.org/onto/class/google_cloud_run_v2_service"/>
    <rdfs:range rdf:resource="http://www.w3.org/2001/XMLSchema#string"/>
  </owl:DatatypeProperty>
  <owl:DatatypeProperty rdf:about="http://example.org/onto/prop/google_cloud_run_v2_service_cpu_idle">
    <rdfs:label>cpu_idle</rdfs:label>
    <rdfs:comment>Determines whether CPU is only allocated during requests. True by default if the parent 'resources' field is not set. However, if
'resources' is set, this field must be explicitly set to true to preserve the default behavior.</rdfs:comment>
    <rdfs:domain rdf:resource="http://example.org/onto/class/google_cloud_run_v2_service"/>
    <rdfs:range rdf:resource="http://www.w3.org/2001/XMLSchema#string"/>
  </owl:DatatypeProperty>
  <owl:DatatypeProperty rdf:about="http://example.org/onto/prop/google_cloud_run_v2_service_limits">
    <rdfs:label>limits</rdfs:label>
    <rdfs:comment>Only memory, CPU, and nvidia.com/gpu are supported. Use key 'cpu' for CPU limit, 'memory' for memory limit, 'nvidia.com/gpu' for gpu limit. Note: The only supported values for CPU are '1', '2', '4', and '8'. Setting 4 CPU requires at least 2Gi of memory. The values of the map is string form of the 'quantity' k8s type: https://github.com/kubernetes/kubernetes/blob/master/staging/src/k8s.io/apimachinery/pkg/api/resource/quantity.go</rdfs:comment>
    <rdfs:domain rdf:resource="http://example.org/onto/class/google_cloud_run_v2_service"/>
    <rdfs:range rdf:resource="http://www.w3.org/2001/XMLSchema#string"/>
  </owl:DatatypeProperty>
  <owl:DatatypeProperty rdf:about="http://example.org/onto/prop/google_cloud_run_v2_service_startup_cpu_boost">
    <rdfs:label>startup_cpu_boost</rdfs:label>
    <rdfs:comment>Determines whether CPU should be boosted on startup of a new container instance above the requested CPU threshold, this can help reduce cold-start latency.</rdfs:comment>
    <rdfs:domain rdf:resource="http://example.org/onto/class/google_cloud_run_v2_service"/>
    <rdfs:range rdf:resource="http://www.w3.org/2001/XMLSchema#string"/>
  </owl:DatatypeProperty>
  <owl:DatatypeProperty rdf:about="http://example.org/onto/prop/google_cloud_run_v2_service_failure_threshold">
    <rdfs:label>failure_threshold</rdfs:label>
    <rdfs:comment>Minimum consecutive failures for the probe to be considered failed after having succeeded. Defaults to 3. Minimum value is 1.</rdfs:comment>
    <rdfs:domain rdf:resource="http://example.org/onto/class/google_cloud_run_v2_service"/>
    <rdfs:range rdf:resource="http://www.w3.org/2001/XMLSchema#string"/>
  </owl:DatatypeProperty>
  <owl:DatatypeProperty rdf:about="http://example.org/onto/prop/google_cloud_run_v2_service_initial_delay_seconds">
    <rdfs:label>initial_delay_seconds</rdfs:label>
    <rdfs:comment>Number of seconds after the container has started before the probe is initiated. Defaults to 0 seconds. Minimum value is 0. Maximum value for liveness probe is 3600. Maximum value for startup probe is 240. More info: https://kubernetes.io/docs/concepts/workloads/pods/pod-lifecycle#container-probes</rdfs:comment>
    <rdfs:domain rdf:resource="http://example.org/onto/class/google_cloud_run_v2_service"/>
    <rdfs:range rdf:resource="http://www.w3.org/2001/XMLSchema#string"/>
  </owl:DatatypeProperty>
  <owl:DatatypeProperty rdf:about="http://example.org/onto/prop/google_cloud_run_v2_service_period_seconds">
    <rdfs:label>period_seconds</rdfs:label>
    <rdfs:comment>How often (in seconds) to perform the probe. Default to 10 seconds. Minimum value is 1. Maximum value for liveness probe is 3600. Maximum value for startup probe is 240. Must be greater or equal than timeoutSeconds</rdfs:comment>
    <rdfs:domain rdf:resource="http://example.org/onto/class/google_cloud_run_v2_service"/>
    <rdfs:range rdf:resource="http://www.w3.org/2001/XMLSchema#string"/>
  </owl:DatatypeProperty>
  <owl:DatatypeProperty rdf:about="http://example.org/onto/prop/google_cloud_run_v2_service_timeout_seconds">
    <rdfs:label>timeout_seconds</rdfs:label>
    <rdfs:comment>Number of seconds after which the probe times out. Defaults to 1 second. Minimum value is 1. Maximum value is 3600. Must be smaller than periodSeconds. More info: https://kubernetes.io/docs/concepts/workloads/pods/pod-lifecycle#container-probes</rdfs:comment>
    <rdfs:domain rdf:resource="http://example.org/onto/class/google_cloud_run_v2_service"/>
    <rdfs:range rdf:resource="http://www.w3.org/2001/XMLSchema#string"/>
  </owl:DatatypeProperty>
  <owl:DatatypeProperty rdf:about="http://example.org/onto/prop/google_cloud_run_v2_service_port">
    <rdfs:label>port</rdfs:label>
    <rdfs:comment>Port number to access on the container. Number must be in the range 1 to 65535.
If not specified, defaults to the same value as container.ports[0].containerPort.</rdfs:comment>
    <rdfs:domain rdf:resource="http://example.org/onto/class/google_cloud_run_v2_service"/>
    <rdfs:range rdf:resource="http://www.w3.org/2001/XMLSchema#string"/>
  </owl:DatatypeProperty>
  <owl:DatatypeProperty rdf:about="http://example.org/onto/prop/google_cloud_run_v2_service_service">
    <rdfs:label>service</rdfs:label>
    <rdfs:comment>The name of the service to place in the gRPC HealthCheckRequest
(see https://github.com/grpc/grpc/blob/master/doc/health-checking.md).
If this is not specified, the default behavior is defined by gRPC.</rdfs:comment>
    <rdfs:domain rdf:resource="http://example.org/onto/class/google_cloud_run_v2_service"/>
    <rdfs:range rdf:resource="http://www.w3.org/2001/XMLSchema#string"/>
  </owl:DatatypeProperty>
  <owl:DatatypeProperty rdf:about="http://example.org/onto/prop/google_cloud_run_v2_service_path">
    <rdfs:label>path</rdfs:label>
    <rdfs:comment>Path to access on the HTTP server. Defaults to '/'.</rdfs:comment>
    <rdfs:domain rdf:resource="http://example.org/onto/class/google_cloud_run_v2_service"/>
    <rdfs:range rdf:resource="http://www.w3.org/2001/XMLSchema#string"/>
  </owl:DatatypeProperty>
  <owl:DatatypeProperty rdf:about="http://example.org/onto/prop/google_cloud_run_v2_service_port">
    <rdfs:label>port</rdfs:label>
    <rdfs:comment>Port number to access on the container. Must be in the range 1 to 65535.
If not specified, defaults to the same value as container.ports[0].containerPort.</rdfs:comment>
    <rdfs:domain rdf:resource="http://example.org/onto/class/google_cloud_run_v2_service"/>
    <rdfs:range rdf:resource="http://www.w3.org/2001/XMLSchema#string"/>
  </owl:DatatypeProperty>
  <owl:DatatypeProperty rdf:about="http://example.org/onto/prop/google_cloud_run_v2_service_name">
    <rdfs:label>name</rdfs:label>
    <rdfs:comment>The header field name</rdfs:comment>
    <rdfs:domain rdf:resource="http://example.org/onto/class/google_cloud_run_v2_service"/>
    <rdfs:range rdf:resource="http://www.w3.org/2001/XMLSchema#string"/>
  </owl:DatatypeProperty>
  <owl:DatatypeProperty rdf:about="http://example.org/onto/prop/google_cloud_run_v2_service_value">
    <rdfs:label>value</rdfs:label>
    <rdfs:comment>The header field value</rdfs:comment>
    <rdfs:domain rdf:resource="http://example.org/onto/class/google_cloud_run_v2_service"/>
    <rdfs:range rdf:resource="http://www.w3.org/2001/XMLSchema#string"/>
  </owl:DatatypeProperty>
  <owl:DatatypeProperty rdf:about="http://example.org/onto/prop/google_cloud_run_v2_service_port">
    <rdfs:label>port</rdfs:label>
    <rdfs:comment>Port number to access on the container. Must be in the range 1 to 65535.
If not specified, defaults to the same value as container.ports[0].containerPort.</rdfs:comment>
    <rdfs:domain rdf:resource="http://example.org/onto/class/google_cloud_run_v2_service"/>
    <rdfs:range rdf:resource="http://www.w3.org/2001/XMLSchema#string"/>
  </owl:DatatypeProperty>
  <owl:DatatypeProperty rdf:about="http://example.org/onto/prop/google_cloud_run_v2_service_mount_path">
    <rdfs:label>mount_path</rdfs:label>
    <rdfs:comment>Path within the container at which the volume should be mounted. Must not contain ':'. For Cloud SQL volumes, it can be left empty, or must otherwise be /cloudsql. All instances defined in the Volume will be available as /cloudsql/[instance]. For more information on Cloud SQL volumes, visit https://cloud.google.com/sql/docs/mysql/connect-run</rdfs:comment>
    <rdfs:domain rdf:resource="http://example.org/onto/class/google_cloud_run_v2_service"/>
    <rdfs:range rdf:resource="http://www.w3.org/2001/XMLSchema#string"/>
  </owl:DatatypeProperty>
  <owl:DatatypeProperty rdf:about="http://example.org/onto/prop/google_cloud_run_v2_service_name">
    <rdfs:label>name</rdfs:label>
    <rdfs:comment>This must match the Name of a Volume.</rdfs:comment>
    <rdfs:domain rdf:resource="http://example.org/onto/class/google_cloud_run_v2_service"/>
    <rdfs:range rdf:resource="http://www.w3.org/2001/XMLSchema#string"/>
  </owl:DatatypeProperty>
  <owl:DatatypeProperty rdf:about="http://example.org/onto/prop/google_cloud_run_v2_service_sub_path">
    <rdfs:label>sub_path</rdfs:label>
    <rdfs:comment>Path within the volume from which the container's volume should be mounted.</rdfs:comment>
    <rdfs:domain rdf:resource="http://example.org/onto/class/google_cloud_run_v2_service"/>
    <rdfs:range rdf:resource="http://www.w3.org/2001/XMLSchema#string"/>
  </owl:DatatypeProperty>
  <owl:DatatypeProperty rdf:about="http://example.org/onto/prop/google_cloud_run_v2_service_accelerator">
    <rdfs:label>accelerator</rdfs:label>
    <rdfs:comment>The GPU to attach to an instance. See https://cloud.google.com/run/docs/configuring/services/gpu for configuring GPU.</rdfs:comment>
    <rdfs:domain rdf:resource="http://example.org/onto/class/google_cloud_run_v2_service"/>
    <rdfs:range rdf:resource="http://www.w3.org/2001/XMLSchema#string"/>
  </owl:DatatypeProperty>
  <owl:DatatypeProperty rdf:about="http://example.org/onto/prop/google_cloud_run_v2_service_max_instance_count">
    <rdfs:label>max_instance_count</rdfs:label>
    <rdfs:comment>Maximum number of serving instances that this resource should have. Must not be less than minimum instance count. If absent, Cloud Run will calculate
a default value based on the project's available container instances quota in the region and specified instance size.</rdfs:comment>
    <rdfs:domain rdf:resource="http://example.org/onto/class/google_cloud_run_v2_service"/>
    <rdfs:range rdf:resource="http://www.w3.org/2001/XMLSchema#string"/>
  </owl:DatatypeProperty>
  <owl:DatatypeProperty rdf:about="http://example.org/onto/prop/google_cloud_run_v2_service_min_instance_count">
    <rdfs:label>min_instance_count</rdfs:label>
    <rdfs:comment>Minimum number of serving instances that this resource should have. Defaults to 0. Must not be greater than maximum instance count.</rdfs:comment>
    <rdfs:domain rdf:resource="http://example.org/onto/class/google_cloud_run_v2_service"/>
    <rdfs:range rdf:resource="http://www.w3.org/2001/XMLSchema#string"/>
  </owl:DatatypeProperty>
  <owl:DatatypeProperty rdf:about="http://example.org/onto/prop/google_cloud_run_v2_service_name">
    <rdfs:label>name</rdfs:label>
    <rdfs:comment>Volume's name.</rdfs:comment>
    <rdfs:domain rdf:resource="http://example.org/onto/class/google_cloud_run_v2_service"/>
    <rdfs:range rdf:resource="http://www.w3.org/2001/XMLSchema#string"/>
  </owl:DatatypeProperty>
  <owl:DatatypeProperty rdf:about="http://example.org/onto/prop/google_cloud_run_v2_service_instances">
    <rdfs:label>instances</rdfs:label>
    <rdfs:comment>The Cloud SQL instance connection names, as can be found in https://console.cloud.google.com/sql/instances. Visit https://cloud.google.com/sql/docs/mysql/connect-run for more information on how to connect Cloud SQL and Cloud Run. Format: {project}:{location}:{instance}</rdfs:comment>
    <rdfs:domain rdf:resource="http://example.org/onto/class/google_cloud_run_v2_service"/>
    <rdfs:range rdf:resource="http://www.w3.org/2001/XMLSchema#string"/>
  </owl:DatatypeProperty>
  <owl:DatatypeProperty rdf:about="http://example.org/onto/prop/google_cloud_run_v2_service_medium">
    <rdfs:label>medium</rdfs:label>
    <rdfs:comment>The different types of medium supported for EmptyDir. Default value: "MEMORY" Possible values: ["MEMORY"]</rdfs:comment>
    <rdfs:domain rdf:resource="http://example.org/onto/class/google_cloud_run_v2_service"/>
    <rdfs:range rdf:resource="http://www.w3.org/2001/XMLSchema#string"/>
  </owl:DatatypeProperty>
  <owl:DatatypeProperty rdf:about="http://example.org/onto/prop/google_cloud_run_v2_service_size_limit">
    <rdfs:label>size_limit</rdfs:label>
    <rdfs:comment>Limit on the storage usable by this EmptyDir volume. The size limit is also applicable for memory medium. The maximum usage on memory medium EmptyDir would be the minimum value between the SizeLimit specified here and the sum of memory limits of all containers in a pod. This field's values are of the 'Quantity' k8s type: https://kubernetes.io/docs/reference/kubernetes-api/common-definitions/quantity/. The default is nil which means that the limit is undefined. More info: https://kubernetes.io/docs/concepts/storage/volumes/#emptydir.</rdfs:comment>
    <rdfs:domain rdf:resource="http://example.org/onto/class/google_cloud_run_v2_service"/>
    <rdfs:range rdf:resource="http://www.w3.org/2001/XMLSchema#string"/>
  </owl:DatatypeProperty>
  <owl:DatatypeProperty rdf:about="http://example.org/onto/prop/google_cloud_run_v2_service_bucket">
    <rdfs:label>bucket</rdfs:label>
    <rdfs:comment>GCS Bucket name</rdfs:comment>
    <rdfs:domain rdf:resource="http://example.org/onto/class/google_cloud_run_v2_service"/>
    <rdfs:range rdf:resource="http://www.w3.org/2001/XMLSchema#string"/>
  </owl:DatatypeProperty>
  <owl:DatatypeProperty rdf:about="http://example.org/onto/prop/google_cloud_run_v2_service_mount_options">
    <rdfs:label>mount_options</rdfs:label>
    <rdfs:comment>A list of flags to pass to the gcsfuse command for configuring this volume.
Flags should be passed without leading dashes.</rdfs:comment>
    <rdfs:domain rdf:resource="http://example.org/onto/class/google_cloud_run_v2_service"/>
    <rdfs:range rdf:resource="http://www.w3.org/2001/XMLSchema#string"/>
  </owl:DatatypeProperty>
  <owl:DatatypeProperty rdf:about="http://example.org/onto/prop/google_cloud_run_v2_service_read_only">
    <rdfs:label>read_only</rdfs:label>
    <rdfs:comment>If true, mount the GCS bucket as read-only</rdfs:comment>
    <rdfs:domain rdf:resource="http://example.org/onto/class/google_cloud_run_v2_service"/>
    <rdfs:range rdf:resource="http://www.w3.org/2001/XMLSchema#string"/>
  </owl:DatatypeProperty>
  <owl:DatatypeProperty rdf:about="http://example.org/onto/prop/google_cloud_run_v2_service_path">
    <rdfs:label>path</rdfs:label>
    <rdfs:comment>Path that is exported by the NFS server.</rdfs:comment>
    <rdfs:domain rdf:resource="http://example.org/onto/class/google_cloud_run_v2_service"/>
    <rdfs:range rdf:resource="http://www.w3.org/2001/XMLSchema#string"/>
  </owl:DatatypeProperty>
  <owl:DatatypeProperty rdf:about="http://example.org/onto/prop/google_cloud_run_v2_service_read_only">
    <rdfs:label>read_only</rdfs:label>
    <rdfs:comment>If true, mount the NFS volume as read only</rdfs:comment>
    <rdfs:domain rdf:resource="http://example.org/onto/class/google_cloud_run_v2_service"/>
    <rdfs:range rdf:resource="http://www.w3.org/2001/XMLSchema#string"/>
  </owl:DatatypeProperty>
  <owl:DatatypeProperty rdf:about="http://example.org/onto/prop/google_cloud_run_v2_service_server">
    <rdfs:label>server</rdfs:label>
    <rdfs:comment>Hostname or IP address of the NFS server</rdfs:comment>
    <rdfs:domain rdf:resource="http://example.org/onto/class/google_cloud_run_v2_service"/>
    <rdfs:range rdf:resource="http://www.w3.org/2001/XMLSchema#string"/>
  </owl:DatatypeProperty>
  <owl:DatatypeProperty rdf:about="http://example.org/onto/prop/google_cloud_run_v2_service_default_mode">
    <rdfs:label>default_mode</rdfs:label>
    <rdfs:comment>Integer representation of mode bits to use on created files by default. Must be a value between 0000 and 0777 (octal), defaulting to 0444. Directories within the path are not affected by this setting.</rdfs:comment>
    <rdfs:domain rdf:resource="http://example.org/onto/class/google_cloud_run_v2_service"/>
    <rdfs:range rdf:resource="http://www.w3.org/2001/XMLSchema#string"/>
  </owl:DatatypeProperty>
  <owl:DatatypeProperty rdf:about="http://example.org/onto/prop/google_cloud_run_v2_service_secret">
    <rdfs:label>secret</rdfs:label>
    <rdfs:comment>The name of the secret in Cloud Secret Manager. Format: {secret} if the secret is in the same project. projects/{project}/secrets/{secret} if the secret is in a different project.</rdfs:comment>
    <rdfs:domain rdf:resource="http://example.org/onto/class/google_cloud_run_v2_service"/>
    <rdfs:range rdf:resource="http://www.w3.org/2001/XMLSchema#string"/>
  </owl:DatatypeProperty>
  <owl:DatatypeProperty rdf:about="http://example.org/onto/prop/google_cloud_run_v2_service_mode">
    <rdfs:label>mode</rdfs:label>
    <rdfs:comment>Integer octal mode bits to use on this file, must be a value between 01 and 0777 (octal). If 0 or not set, the Volume's default mode will be used.</rdfs:comment>
    <rdfs:domain rdf:resource="http://example.org/onto/class/google_cloud_run_v2_service"/>
    <rdfs:range rdf:resource="http://www.w3.org/2001/XMLSchema#string"/>
  </owl:DatatypeProperty>
  <owl:DatatypeProperty rdf:about="http://example.org/onto/prop/google_cloud_run_v2_service_path">
    <rdfs:label>path</rdfs:label>
    <rdfs:comment>The relative path of the secret in the container.</rdfs:comment>
    <rdfs:domain rdf:resource="http://example.org/onto/class/google_cloud_run_v2_service"/>
    <rdfs:range rdf:resource="http://www.w3.org/2001/XMLSchema#string"/>
  </owl:DatatypeProperty>
  <owl:DatatypeProperty rdf:about="http://example.org/onto/prop/google_cloud_run_v2_service_version">
    <rdfs:label>version</rdfs:label>
    <rdfs:comment>The Cloud Secret Manager secret version. Can be 'latest' for the latest value or an integer for a specific version</rdfs:comment>
    <rdfs:domain rdf:resource="http://example.org/onto/class/google_cloud_run_v2_service"/>
    <rdfs:range rdf:resource="http://www.w3.org/2001/XMLSchema#string"/>
  </owl:DatatypeProperty>
  <owl:DatatypeProperty rdf:about="http://example.org/onto/prop/google_cloud_run_v2_service_connector">
    <rdfs:label>connector</rdfs:label>
    <rdfs:comment>VPC Access connector name. Format: projects/{project}/locations/{location}/connectors/{connector}, where {project} can be project id or number.</rdfs:comment>
    <rdfs:domain rdf:resource="http://example.org/onto/class/google_cloud_run_v2_service"/>
    <rdfs:range rdf:resource="http://www.w3.org/2001/XMLSchema#string"/>
  </owl:DatatypeProperty>
  <owl:DatatypeProperty rdf:about="http://example.org/onto/prop/google_cloud_run_v2_service_egress">
    <rdfs:label>egress</rdfs:label>
    <rdfs:comment>Traffic VPC egress settings. Possible values: ["ALL_TRAFFIC", "PRIVATE_RANGES_ONLY"]</rdfs:comment>
    <rdfs:domain rdf:resource="http://example.org/onto/class/google_cloud_run_v2_service"/>
    <rdfs:range rdf:resource="http://www.w3.org/2001/XMLSchema#string"/>
  </owl:DatatypeProperty>
  <owl:DatatypeProperty rdf:about="http://example.org/onto/prop/google_cloud_run_v2_service_network">
    <rdfs:label>network</rdfs:label>
    <rdfs:comment>The VPC network that the Cloud Run resource will be able to send traffic to. At least one of network or subnetwork must be specified. If both
network and subnetwork are specified, the given VPC subnetwork must belong to the given VPC network. If network is not specified, it will be
looked up from the subnetwork.</rdfs:comment>
    <rdfs:domain rdf:resource="http://example.org/onto/class/google_cloud_run_v2_service"/>
    <rdfs:range rdf:resource="http://www.w3.org/2001/XMLSchema#string"/>
  </owl:DatatypeProperty>
  <owl:DatatypeProperty rdf:about="http://example.org/onto/prop/google_cloud_run_v2_service_subnetwork">
    <rdfs:label>subnetwork</rdfs:label>
    <rdfs:comment>The VPC subnetwork that the Cloud Run resource will get IPs from. At least one of network or subnetwork must be specified. If both
network and subnetwork are specified, the given VPC subnetwork must belong to the given VPC network. If subnetwork is not specified, the
subnetwork with the same name with the network will be used.</rdfs:comment>
    <rdfs:domain rdf:resource="http://example.org/onto/class/google_cloud_run_v2_service"/>
    <rdfs:range rdf:resource="http://www.w3.org/2001/XMLSchema#string"/>
  </owl:DatatypeProperty>
  <owl:DatatypeProperty rdf:about="http://example.org/onto/prop/google_cloud_run_v2_service_tags">
    <rdfs:label>tags</rdfs:label>
    <rdfs:comment>Network tags applied to this Cloud Run service.</rdfs:comment>
    <rdfs:domain rdf:resource="http://example.org/onto/class/google_cloud_run_v2_service"/>
    <rdfs:range rdf:resource="http://www.w3.org/2001/XMLSchema#string"/>
  </owl:DatatypeProperty>
  <owl:DatatypeProperty rdf:about="http://example.org/onto/prop/google_cloud_run_v2_service_create">
    <rdfs:label>create</rdfs:label>
    <rdfs:domain rdf:resource="http://example.org/onto/class/google_cloud_run_v2_service"/>
    <rdfs:range rdf:resource="http://www.w3.org/2001/XMLSchema#string"/>
  </owl:DatatypeProperty>
  <owl:DatatypeProperty rdf:about="http://example.org/onto/prop/google_cloud_run_v2_service_delete">
    <rdfs:label>delete</rdfs:label>
    <rdfs:domain rdf:resource="http://example.org/onto/class/google_cloud_run_v2_service"/>
    <rdfs:range rdf:resource="http://www.w3.org/2001/XMLSchema#string"/>
  </owl:DatatypeProperty>
  <owl:DatatypeProperty rdf:about="http://example.org/onto/prop/google_cloud_run_v2_service_update">
    <rdfs:label>update</rdfs:label>
    <rdfs:domain rdf:resource="http://example.org/onto/class/google_cloud_run_v2_service"/>
    <rdfs:range rdf:resource="http://www.w3.org/2001/XMLSchema#string"/>
  </owl:DatatypeProperty>
  <owl:DatatypeProperty rdf:about="http://example.org/onto/prop/google_cloud_run_v2_service_percent">
    <rdfs:label>percent</rdfs:label>
    <rdfs:comment>Specifies percent of the traffic to this Revision. This defaults to zero if unspecified.</rdfs:comment>
    <rdfs:domain rdf:resource="http://example.org/onto/class/google_cloud_run_v2_service"/>
    <rdfs:range rdf:resource="http://www.w3.org/2001/XMLSchema#string"/>
  </owl:DatatypeProperty>
  <owl:DatatypeProperty rdf:about="http://example.org/onto/prop/google_cloud_run_v2_service_revision">
    <rdfs:label>revision</rdfs:label>
    <rdfs:comment>Revision to which to send this portion of traffic, if traffic allocation is by revision.</rdfs:comment>
    <rdfs:domain rdf:resource="http://example.org/onto/class/google_cloud_run_v2_service"/>
    <rdfs:range rdf:resource="http://www.w3.org/2001/XMLSchema#string"/>
  </owl:DatatypeProperty>
  <owl:DatatypeProperty rdf:about="http://example.org/onto/prop/google_cloud_run_v2_service_tag">
    <rdfs:label>tag</rdfs:label>
    <rdfs:comment>Indicates a string to be part of the URI to exclusively reference this target.</rdfs:comment>
    <rdfs:domain rdf:resource="http://example.org/onto/class/google_cloud_run_v2_service"/>
    <rdfs:range rdf:resource="http://www.w3.org/2001/XMLSchema#string"/>
  </owl:DatatypeProperty>
  <owl:DatatypeProperty rdf:about="http://example.org/onto/prop/google_cloud_run_v2_service_type">
    <rdfs:label>type</rdfs:label>
    <rdfs:comment>The allocation type for this traffic target. Possible values: ["TRAFFIC_TARGET_ALLOCATION_TYPE_LATEST", "TRAFFIC_TARGET_ALLOCATION_TYPE_REVISION"]</rdfs:comment>
    <rdfs:domain rdf:resource="http://example.org/onto/class/google_cloud_run_v2_service"/>
    <rdfs:range rdf:resource="http://www.w3.org/2001/XMLSchema#string"/>
  </owl:DatatypeProperty>
</rdf:RDF>
