<?xml version="1.0" encoding="UTF-8"?>
<rdf:RDF
  xmlns:rdf="http://www.w3.org/1999/02/22-rdf-syntax-ns#"
  xmlns:rdfs="http://www.w3.org/2000/01/rdf-schema#"
  xmlns:owl="http://www.w3.org/2002/07/owl#"
  xmlns:xsd="http://www.w3.org/2001/XMLSchema#"
  xml:base="http://example.org/onto/">
  <owl:Class rdf:about="http://example.org/onto/class/google_access_context_manager_service_perimeter_dry_run_egress_policy">
    <rdfs:label>google_access_context_manager_service_perimeter_dry_run_egress_policy</rdfs:label>
    <rdfs:comment>#
#     ***     AUTO GENERATED CODE    ***    Type: MMv1     ***
#
# ----------------------------------------------------------------------------
#
#     This code is generated by Magic Modules using the following:
#
#     Configuration: https:#github.com/GoogleCloudPlatform/magic-modules/tree/main/mmv1/products/accesscontextmanager/ServicePerimeterDryRunEgressPolicy.yaml
#     Template:      https:#github.com/GoogleCloudPlatform/magic-modules/tree/main/mmv1/templates/terraform/resource.html.markdown.tmpl
#
#     DO NOT EDIT this file directly. Any changes made to this file will be
#     overwritten during the next generation cycle.
#
# ----------------------------------------------------------------------------
subcategory: "Access Context Manager (VPC Service Controls)"
description: |-
  Manage a single EgressPolicy in the spec (dry-run) configuration for a service perimeter.
---</rdfs:comment>
  </owl:Class>
  <owl:DatatypeProperty rdf:about="http://example.org/onto/prop/google_access_context_manager_service_perimeter_dry_run_egress_policy_access_policy_id">
    <rdfs:label>access_policy_id</rdfs:label>
    <rdfs:comment>The name of the Access Policy this resource belongs to.</rdfs:comment>
    <rdfs:domain rdf:resource="http://example.org/onto/class/google_access_context_manager_service_perimeter_dry_run_egress_policy"/>
    <rdfs:range rdf:resource="http://www.w3.org/2001/XMLSchema#string"/>
  </owl:DatatypeProperty>
  <owl:DatatypeProperty rdf:about="http://example.org/onto/prop/google_access_context_manager_service_perimeter_dry_run_egress_policy_etag">
    <rdfs:label>etag</rdfs:label>
    <rdfs:comment>The perimeter etag is internally used to prevent overwriting the list of policies on PATCH calls. It is retrieved from the same GET perimeter API call that's used to get the current list of policies. The policy defined in this resource is added or removed from that list, and then this etag is sent with the PATCH call along with the updated policies.</rdfs:comment>
    <rdfs:domain rdf:resource="http://example.org/onto/class/google_access_context_manager_service_perimeter_dry_run_egress_policy"/>
    <rdfs:range rdf:resource="http://www.w3.org/2001/XMLSchema#string"/>
  </owl:DatatypeProperty>
  <owl:DatatypeProperty rdf:about="http://example.org/onto/prop/google_access_context_manager_service_perimeter_dry_run_egress_policy_id">
    <rdfs:label>id</rdfs:label>
    <rdfs:domain rdf:resource="http://example.org/onto/class/google_access_context_manager_service_perimeter_dry_run_egress_policy"/>
    <rdfs:range rdf:resource="http://www.w3.org/2001/XMLSchema#string"/>
  </owl:DatatypeProperty>
  <owl:DatatypeProperty rdf:about="http://example.org/onto/prop/google_access_context_manager_service_perimeter_dry_run_egress_policy_perimeter">
    <rdfs:label>perimeter</rdfs:label>
    <rdfs:comment>The name of the Service Perimeter to add this resource to.</rdfs:comment>
    <rdfs:domain rdf:resource="http://example.org/onto/class/google_access_context_manager_service_perimeter_dry_run_egress_policy"/>
    <rdfs:range rdf:resource="http://www.w3.org/2001/XMLSchema#string"/>
  </owl:DatatypeProperty>
  <owl:DatatypeProperty rdf:about="http://example.org/onto/prop/google_access_context_manager_service_perimeter_dry_run_egress_policy_title">
    <rdfs:label>title</rdfs:label>
    <rdfs:comment>Human readable title. Must be unique within the perimeter. Does not affect behavior.</rdfs:comment>
    <rdfs:domain rdf:resource="http://example.org/onto/class/google_access_context_manager_service_perimeter_dry_run_egress_policy"/>
    <rdfs:range rdf:resource="http://www.w3.org/2001/XMLSchema#string"/>
  </owl:DatatypeProperty>
  <owl:DatatypeProperty rdf:about="http://example.org/onto/prop/google_access_context_manager_service_perimeter_dry_run_egress_policy_identities">
    <rdfs:label>identities</rdfs:label>
    <rdfs:comment>Identities can be an individual user, service account, Google group,
or third-party identity. For third-party identity, only single identities
are supported and other identity types are not supported.The v1 identities
that have the prefix user, group and serviceAccount in
https://cloud.google.com/iam/docs/principal-identifiers#v1 are supported.</rdfs:comment>
    <rdfs:domain rdf:resource="http://example.org/onto/class/google_access_context_manager_service_perimeter_dry_run_egress_policy"/>
    <rdfs:range rdf:resource="http://www.w3.org/2001/XMLSchema#string"/>
  </owl:DatatypeProperty>
  <owl:DatatypeProperty rdf:about="http://example.org/onto/prop/google_access_context_manager_service_perimeter_dry_run_egress_policy_identity_type">
    <rdfs:label>identity_type</rdfs:label>
    <rdfs:comment>Specifies the type of identities that are allowed access to outside the
perimeter. If left unspecified, then members of 'identities' field will
be allowed access. Possible values: ["ANY_IDENTITY", "ANY_USER_ACCOUNT", "ANY_SERVICE_ACCOUNT"]</rdfs:comment>
    <rdfs:domain rdf:resource="http://example.org/onto/class/google_access_context_manager_service_perimeter_dry_run_egress_policy"/>
    <rdfs:range rdf:resource="http://www.w3.org/2001/XMLSchema#string"/>
  </owl:DatatypeProperty>
  <owl:DatatypeProperty rdf:about="http://example.org/onto/prop/google_access_context_manager_service_perimeter_dry_run_egress_policy_source_restriction">
    <rdfs:label>source_restriction</rdfs:label>
    <rdfs:comment>Whether to enforce traffic restrictions based on 'sources' field. If the 'sources' field is non-empty, then this field must be set to 'SOURCE_RESTRICTION_ENABLED'. Possible values: ["SOURCE_RESTRICTION_ENABLED", "SOURCE_RESTRICTION_DISABLED"]</rdfs:comment>
    <rdfs:domain rdf:resource="http://example.org/onto/class/google_access_context_manager_service_perimeter_dry_run_egress_policy"/>
    <rdfs:range rdf:resource="http://www.w3.org/2001/XMLSchema#string"/>
  </owl:DatatypeProperty>
  <owl:DatatypeProperty rdf:about="http://example.org/onto/prop/google_access_context_manager_service_perimeter_dry_run_egress_policy_access_level">
    <rdfs:label>access_level</rdfs:label>
    <rdfs:comment>An AccessLevel resource name that allows resources outside the ServicePerimeter to be accessed from the inside.</rdfs:comment>
    <rdfs:domain rdf:resource="http://example.org/onto/class/google_access_context_manager_service_perimeter_dry_run_egress_policy"/>
    <rdfs:range rdf:resource="http://www.w3.org/2001/XMLSchema#string"/>
  </owl:DatatypeProperty>
  <owl:DatatypeProperty rdf:about="http://example.org/onto/prop/google_access_context_manager_service_perimeter_dry_run_egress_policy_resource">
    <rdfs:label>resource</rdfs:label>
    <rdfs:comment>A Google Cloud resource that is allowed to egress the perimeter.
Requests from these resources are allowed to access data outside the perimeter.
Currently only projects are allowed. Project format: 'projects/{project_number}'.
The resource may be in any Google Cloud organization, not just the
organization that the perimeter is defined in. '*' is not allowed, the
case of allowing all Google Cloud resources only is not supported.</rdfs:comment>
    <rdfs:domain rdf:resource="http://example.org/onto/class/google_access_context_manager_service_perimeter_dry_run_egress_policy"/>
    <rdfs:range rdf:resource="http://www.w3.org/2001/XMLSchema#string"/>
  </owl:DatatypeProperty>
  <owl:DatatypeProperty rdf:about="http://example.org/onto/prop/google_access_context_manager_service_perimeter_dry_run_egress_policy_external_resources">
    <rdfs:label>external_resources</rdfs:label>
    <rdfs:comment>A list of external resources that are allowed to be accessed. A request
matches if it contains an external resource in this list (Example:
s3://bucket/path). Currently '*' is not allowed.</rdfs:comment>
    <rdfs:domain rdf:resource="http://example.org/onto/class/google_access_context_manager_service_perimeter_dry_run_egress_policy"/>
    <rdfs:range rdf:resource="http://www.w3.org/2001/XMLSchema#string"/>
  </owl:DatatypeProperty>
  <owl:DatatypeProperty rdf:about="http://example.org/onto/prop/google_access_context_manager_service_perimeter_dry_run_egress_policy_resources">
    <rdfs:label>resources</rdfs:label>
    <rdfs:comment>A list of resources, currently only projects in the form
'projects/<projectnumber>', that match this to stanza. A request matches
if it contains a resource in this list. If * is specified for resources,
then this 'EgressTo' rule will authorize access to all resources outside
the perimeter.</rdfs:comment>
    <rdfs:domain rdf:resource="http://example.org/onto/class/google_access_context_manager_service_perimeter_dry_run_egress_policy"/>
    <rdfs:range rdf:resource="http://www.w3.org/2001/XMLSchema#string"/>
  </owl:DatatypeProperty>
  <owl:DatatypeProperty rdf:about="http://example.org/onto/prop/google_access_context_manager_service_perimeter_dry_run_egress_policy_roles">
    <rdfs:label>roles</rdfs:label>
    <rdfs:comment>A list of IAM roles that represent the set of operations that the sources
specified in the corresponding 'EgressFrom'
are allowed to perform.</rdfs:comment>
    <rdfs:domain rdf:resource="http://example.org/onto/class/google_access_context_manager_service_perimeter_dry_run_egress_policy"/>
    <rdfs:range rdf:resource="http://www.w3.org/2001/XMLSchema#string"/>
  </owl:DatatypeProperty>
  <owl:DatatypeProperty rdf:about="http://example.org/onto/prop/google_access_context_manager_service_perimeter_dry_run_egress_policy_service_name">
    <rdfs:label>service_name</rdfs:label>
    <rdfs:comment>The name of the API whose methods or permissions the 'IngressPolicy' or
'EgressPolicy' want to allow. A single 'ApiOperation' with serviceName
field set to '*' will allow all methods AND permissions for all services.</rdfs:comment>
    <rdfs:domain rdf:resource="http://example.org/onto/class/google_access_context_manager_service_perimeter_dry_run_egress_policy"/>
    <rdfs:range rdf:resource="http://www.w3.org/2001/XMLSchema#string"/>
  </owl:DatatypeProperty>
  <owl:DatatypeProperty rdf:about="http://example.org/onto/prop/google_access_context_manager_service_perimeter_dry_run_egress_policy_method">
    <rdfs:label>method</rdfs:label>
    <rdfs:comment>Value for 'method' should be a valid method name for the corresponding
'serviceName' in 'ApiOperation'. If '*' used as value for method,
then ALL methods and permissions are allowed.</rdfs:comment>
    <rdfs:domain rdf:resource="http://example.org/onto/class/google_access_context_manager_service_perimeter_dry_run_egress_policy"/>
    <rdfs:range rdf:resource="http://www.w3.org/2001/XMLSchema#string"/>
  </owl:DatatypeProperty>
  <owl:DatatypeProperty rdf:about="http://example.org/onto/prop/google_access_context_manager_service_perimeter_dry_run_egress_policy_permission">
    <rdfs:label>permission</rdfs:label>
    <rdfs:comment>Value for permission should be a valid Cloud IAM permission for the
corresponding 'serviceName' in 'ApiOperation'.</rdfs:comment>
    <rdfs:domain rdf:resource="http://example.org/onto/class/google_access_context_manager_service_perimeter_dry_run_egress_policy"/>
    <rdfs:range rdf:resource="http://www.w3.org/2001/XMLSchema#string"/>
  </owl:DatatypeProperty>
  <owl:DatatypeProperty rdf:about="http://example.org/onto/prop/google_access_context_manager_service_perimeter_dry_run_egress_policy_create">
    <rdfs:label>create</rdfs:label>
    <rdfs:domain rdf:resource="http://example.org/onto/class/google_access_context_manager_service_perimeter_dry_run_egress_policy"/>
    <rdfs:range rdf:resource="http://www.w3.org/2001/XMLSchema#string"/>
  </owl:DatatypeProperty>
  <owl:DatatypeProperty rdf:about="http://example.org/onto/prop/google_access_context_manager_service_perimeter_dry_run_egress_policy_delete">
    <rdfs:label>delete</rdfs:label>
    <rdfs:domain rdf:resource="http://example.org/onto/class/google_access_context_manager_service_perimeter_dry_run_egress_policy"/>
    <rdfs:range rdf:resource="http://www.w3.org/2001/XMLSchema#string"/>
  </owl:DatatypeProperty>
</rdf:RDF>
