<?xml version="1.0" encoding="UTF-8"?>
<rdf:RDF
  xmlns:rdf="http://www.w3.org/1999/02/22-rdf-syntax-ns#"
  xmlns:rdfs="http://www.w3.org/2000/01/rdf-schema#"
  xmlns:owl="http://www.w3.org/2002/07/owl#"
  xmlns:xsd="http://www.w3.org/2001/XMLSchema#"
  xml:base="http://example.org/onto/">
  <owl:Class rdf:about="http://example.org/onto/class/google_dataproc_metastore_federation">
    <rdfs:label>google_dataproc_metastore_federation</rdfs:label>
    <rdfs:comment>#
#     ***     AUTO GENERATED CODE    ***    Type: MMv1     ***
#
# ----------------------------------------------------------------------------
#
#     This code is generated by Magic Modules using the following:
#
#     Configuration: https:#github.com/GoogleCloudPlatform/magic-modules/tree/main/mmv1/products/metastore/Federation.yaml
#     Template:      https:#github.com/GoogleCloudPlatform/magic-modules/tree/main/mmv1/templates/terraform/resource.html.markdown.tmpl
#
#     DO NOT EDIT this file directly. Any changes made to this file will be
#     overwritten during the next generation cycle.
#
# ----------------------------------------------------------------------------
subcategory: "Dataproc Metastore"
description: |-
  A managed metastore federation.
---</rdfs:comment>
  </owl:Class>
  <owl:DatatypeProperty rdf:about="http://example.org/onto/prop/google_dataproc_metastore_federation_create_time">
    <rdfs:label>create_time</rdfs:label>
    <rdfs:comment>Output only. The time when the metastore federation was created.</rdfs:comment>
    <rdfs:domain rdf:resource="http://example.org/onto/class/google_dataproc_metastore_federation"/>
    <rdfs:range rdf:resource="http://www.w3.org/2001/XMLSchema#string"/>
  </owl:DatatypeProperty>
  <owl:DatatypeProperty rdf:about="http://example.org/onto/prop/google_dataproc_metastore_federation_deletion_protection">
    <rdfs:label>deletion_protection</rdfs:label>
    <rdfs:comment>Whether Terraform will be prevented from destroying the federation. Defaults to false.
When the field is set to true in Terraform state, a 'terraform apply'
or 'terraform destroy' that would delete the federation will fail.</rdfs:comment>
    <rdfs:domain rdf:resource="http://example.org/onto/class/google_dataproc_metastore_federation"/>
    <rdfs:range rdf:resource="http://www.w3.org/2001/XMLSchema#string"/>
  </owl:DatatypeProperty>
  <owl:DatatypeProperty rdf:about="http://example.org/onto/prop/google_dataproc_metastore_federation_effective_labels">
    <rdfs:label>effective_labels</rdfs:label>
    <rdfs:comment>All of labels (key/value pairs) present on the resource in GCP, including the labels configured through Terraform, other clients and services.</rdfs:comment>
    <rdfs:domain rdf:resource="http://example.org/onto/class/google_dataproc_metastore_federation"/>
    <rdfs:range rdf:resource="http://www.w3.org/2001/XMLSchema#string"/>
  </owl:DatatypeProperty>
  <owl:DatatypeProperty rdf:about="http://example.org/onto/prop/google_dataproc_metastore_federation_endpoint_uri">
    <rdfs:label>endpoint_uri</rdfs:label>
    <rdfs:comment>The URI of the endpoint used to access the metastore federation.</rdfs:comment>
    <rdfs:domain rdf:resource="http://example.org/onto/class/google_dataproc_metastore_federation"/>
    <rdfs:range rdf:resource="http://www.w3.org/2001/XMLSchema#string"/>
  </owl:DatatypeProperty>
  <owl:DatatypeProperty rdf:about="http://example.org/onto/prop/google_dataproc_metastore_federation_federation_id">
    <rdfs:label>federation_id</rdfs:label>
    <rdfs:comment>The ID of the metastore federation. The id must contain only letters (a-z, A-Z), numbers (0-9), underscores (_),
and hyphens (-). Cannot begin or end with underscore or hyphen. Must consist of between
3 and 63 characters.</rdfs:comment>
    <rdfs:domain rdf:resource="http://example.org/onto/class/google_dataproc_metastore_federation"/>
    <rdfs:range rdf:resource="http://www.w3.org/2001/XMLSchema#string"/>
  </owl:DatatypeProperty>
  <owl:DatatypeProperty rdf:about="http://example.org/onto/prop/google_dataproc_metastore_federation_id">
    <rdfs:label>id</rdfs:label>
    <rdfs:domain rdf:resource="http://example.org/onto/class/google_dataproc_metastore_federation"/>
    <rdfs:range rdf:resource="http://www.w3.org/2001/XMLSchema#string"/>
  </owl:DatatypeProperty>
  <owl:DatatypeProperty rdf:about="http://example.org/onto/prop/google_dataproc_metastore_federation_labels">
    <rdfs:label>labels</rdfs:label>
    <rdfs:comment>User-defined labels for the metastore federation.

**Note**: This field is non-authoritative, and will only manage the labels present in your configuration.
Please refer to the field 'effective_labels' for all of the labels present on the resource.</rdfs:comment>
    <rdfs:domain rdf:resource="http://example.org/onto/class/google_dataproc_metastore_federation"/>
    <rdfs:range rdf:resource="http://www.w3.org/2001/XMLSchema#string"/>
  </owl:DatatypeProperty>
  <owl:DatatypeProperty rdf:about="http://example.org/onto/prop/google_dataproc_metastore_federation_location">
    <rdfs:label>location</rdfs:label>
    <rdfs:comment>The location where the metastore federation should reside.</rdfs:comment>
    <rdfs:domain rdf:resource="http://example.org/onto/class/google_dataproc_metastore_federation"/>
    <rdfs:range rdf:resource="http://www.w3.org/2001/XMLSchema#string"/>
  </owl:DatatypeProperty>
  <owl:DatatypeProperty rdf:about="http://example.org/onto/prop/google_dataproc_metastore_federation_name">
    <rdfs:label>name</rdfs:label>
    <rdfs:comment>The relative resource name of the metastore federation.</rdfs:comment>
    <rdfs:domain rdf:resource="http://example.org/onto/class/google_dataproc_metastore_federation"/>
    <rdfs:range rdf:resource="http://www.w3.org/2001/XMLSchema#string"/>
  </owl:DatatypeProperty>
  <owl:DatatypeProperty rdf:about="http://example.org/onto/prop/google_dataproc_metastore_federation_project">
    <rdfs:label>project</rdfs:label>
    <rdfs:domain rdf:resource="http://example.org/onto/class/google_dataproc_metastore_federation"/>
    <rdfs:range rdf:resource="http://www.w3.org/2001/XMLSchema#string"/>
  </owl:DatatypeProperty>
  <owl:DatatypeProperty rdf:about="http://example.org/onto/prop/google_dataproc_metastore_federation_state">
    <rdfs:label>state</rdfs:label>
    <rdfs:comment>The current state of the metastore federation.</rdfs:comment>
    <rdfs:domain rdf:resource="http://example.org/onto/class/google_dataproc_metastore_federation"/>
    <rdfs:range rdf:resource="http://www.w3.org/2001/XMLSchema#string"/>
  </owl:DatatypeProperty>
  <owl:DatatypeProperty rdf:about="http://example.org/onto/prop/google_dataproc_metastore_federation_state_message">
    <rdfs:label>state_message</rdfs:label>
    <rdfs:comment>Additional information about the current state of the metastore federation, if available.</rdfs:comment>
    <rdfs:domain rdf:resource="http://example.org/onto/class/google_dataproc_metastore_federation"/>
    <rdfs:range rdf:resource="http://www.w3.org/2001/XMLSchema#string"/>
  </owl:DatatypeProperty>
  <owl:DatatypeProperty rdf:about="http://example.org/onto/prop/google_dataproc_metastore_federation_tags">
    <rdfs:label>tags</rdfs:label>
    <rdfs:comment>A map of resource manager tags.
Resource manager tag keys and values have the same definition as resource manager tags.
Keys must be in the format tagKeys/{tag_key_id}, and values are in the format tagValues/{tag_value_id}.</rdfs:comment>
    <rdfs:domain rdf:resource="http://example.org/onto/class/google_dataproc_metastore_federation"/>
    <rdfs:range rdf:resource="http://www.w3.org/2001/XMLSchema#string"/>
  </owl:DatatypeProperty>
  <owl:DatatypeProperty rdf:about="http://example.org/onto/prop/google_dataproc_metastore_federation_terraform_labels">
    <rdfs:label>terraform_labels</rdfs:label>
    <rdfs:comment>The combination of labels configured directly on the resource
 and default labels configured on the provider.</rdfs:comment>
    <rdfs:domain rdf:resource="http://example.org/onto/class/google_dataproc_metastore_federation"/>
    <rdfs:range rdf:resource="http://www.w3.org/2001/XMLSchema#string"/>
  </owl:DatatypeProperty>
  <owl:DatatypeProperty rdf:about="http://example.org/onto/prop/google_dataproc_metastore_federation_uid">
    <rdfs:label>uid</rdfs:label>
    <rdfs:comment>The globally unique resource identifier of the metastore federation.</rdfs:comment>
    <rdfs:domain rdf:resource="http://example.org/onto/class/google_dataproc_metastore_federation"/>
    <rdfs:range rdf:resource="http://www.w3.org/2001/XMLSchema#string"/>
  </owl:DatatypeProperty>
  <owl:DatatypeProperty rdf:about="http://example.org/onto/prop/google_dataproc_metastore_federation_update_time">
    <rdfs:label>update_time</rdfs:label>
    <rdfs:comment>Output only. The time when the metastore federation was last updated.</rdfs:comment>
    <rdfs:domain rdf:resource="http://example.org/onto/class/google_dataproc_metastore_federation"/>
    <rdfs:range rdf:resource="http://www.w3.org/2001/XMLSchema#string"/>
  </owl:DatatypeProperty>
  <owl:DatatypeProperty rdf:about="http://example.org/onto/prop/google_dataproc_metastore_federation_version">
    <rdfs:label>version</rdfs:label>
    <rdfs:comment>The Apache Hive metastore version of the federation. All backend metastore versions must be compatible with the federation version.</rdfs:comment>
    <rdfs:domain rdf:resource="http://example.org/onto/class/google_dataproc_metastore_federation"/>
    <rdfs:range rdf:resource="http://www.w3.org/2001/XMLSchema#string"/>
  </owl:DatatypeProperty>
  <owl:DatatypeProperty rdf:about="http://example.org/onto/prop/google_dataproc_metastore_federation_metastore_type">
    <rdfs:label>metastore_type</rdfs:label>
    <rdfs:comment>The type of the backend metastore. Possible values: ["METASTORE_TYPE_UNSPECIFIED", "DATAPROC_METASTORE", "BIGQUERY"]</rdfs:comment>
    <rdfs:domain rdf:resource="http://example.org/onto/class/google_dataproc_metastore_federation"/>
    <rdfs:range rdf:resource="http://www.w3.org/2001/XMLSchema#string"/>
  </owl:DatatypeProperty>
  <owl:DatatypeProperty rdf:about="http://example.org/onto/prop/google_dataproc_metastore_federation_name">
    <rdfs:label>name</rdfs:label>
    <rdfs:comment>The relative resource name of the metastore that is being federated. The formats of the relative resource names for the currently supported metastores are listed below: Dataplex: projects/{projectId}/locations/{location}/lakes/{lake_id} BigQuery: projects/{projectId} Dataproc Metastore: projects/{projectId}/locations/{location}/services/{serviceId}</rdfs:comment>
    <rdfs:domain rdf:resource="http://example.org/onto/class/google_dataproc_metastore_federation"/>
    <rdfs:range rdf:resource="http://www.w3.org/2001/XMLSchema#string"/>
  </owl:DatatypeProperty>
  <owl:DatatypeProperty rdf:about="http://example.org/onto/prop/google_dataproc_metastore_federation_rank">
    <rdfs:label>rank</rdfs:label>
    <rdfs:domain rdf:resource="http://example.org/onto/class/google_dataproc_metastore_federation"/>
    <rdfs:range rdf:resource="http://www.w3.org/2001/XMLSchema#string"/>
  </owl:DatatypeProperty>
  <owl:DatatypeProperty rdf:about="http://example.org/onto/prop/google_dataproc_metastore_federation_create">
    <rdfs:label>create</rdfs:label>
    <rdfs:domain rdf:resource="http://example.org/onto/class/google_dataproc_metastore_federation"/>
    <rdfs:range rdf:resource="http://www.w3.org/2001/XMLSchema#string"/>
  </owl:DatatypeProperty>
  <owl:DatatypeProperty rdf:about="http://example.org/onto/prop/google_dataproc_metastore_federation_delete">
    <rdfs:label>delete</rdfs:label>
    <rdfs:domain rdf:resource="http://example.org/onto/class/google_dataproc_metastore_federation"/>
    <rdfs:range rdf:resource="http://www.w3.org/2001/XMLSchema#string"/>
  </owl:DatatypeProperty>
  <owl:DatatypeProperty rdf:about="http://example.org/onto/prop/google_dataproc_metastore_federation_update">
    <rdfs:label>update</rdfs:label>
    <rdfs:domain rdf:resource="http://example.org/onto/class/google_dataproc_metastore_federation"/>
    <rdfs:range rdf:resource="http://www.w3.org/2001/XMLSchema#string"/>
  </owl:DatatypeProperty>
</rdf:RDF>
