<?xml version="1.0" encoding="UTF-8"?>
<rdf:RDF
  xmlns:rdf="http://www.w3.org/1999/02/22-rdf-syntax-ns#"
  xmlns:rdfs="http://www.w3.org/2000/01/rdf-schema#"
  xmlns:owl="http://www.w3.org/2002/07/owl#"
  xmlns:xsd="http://www.w3.org/2001/XMLSchema#"
  xml:base="http://example.org/onto/">
  <owl:Class rdf:about="http://example.org/onto/class/google_developer_connect_insights_config">
    <rdfs:label>google_developer_connect_insights_config</rdfs:label>
    <rdfs:comment>#
#     ***     AUTO GENERATED CODE    ***    Type: MMv1     ***
#
# ----------------------------------------------------------------------------
#
#     This code is generated by Magic Modules using the following:
#
#     Configuration: https:#github.com/GoogleCloudPlatform/magic-modules/tree/main/mmv1/products/developerconnect/InsightsConfig.yaml
#     Template:      https:#github.com/GoogleCloudPlatform/magic-modules/tree/main/mmv1/templates/terraform/resource.html.markdown.tmpl
#
#     DO NOT EDIT this file directly. Any changes made to this file will be
#     overwritten during the next generation cycle.
#
# ----------------------------------------------------------------------------
subcategory: "Developer Connect"
description: |-
  Description
---</rdfs:comment>
  </owl:Class>
  <owl:DatatypeProperty rdf:about="http://example.org/onto/prop/google_developer_connect_insights_config_annotations">
    <rdfs:label>annotations</rdfs:label>
    <rdfs:comment>User specified annotations. See https://google.aip.dev/148#annotations
for more details such as format and size limitations.

**Note**: This field is non-authoritative, and will only manage the annotations present in your configuration.
Please refer to the field 'effective_annotations' for all of the annotations present on the resource.</rdfs:comment>
    <rdfs:domain rdf:resource="http://example.org/onto/class/google_developer_connect_insights_config"/>
    <rdfs:range rdf:resource="http://www.w3.org/2001/XMLSchema#string"/>
  </owl:DatatypeProperty>
  <owl:DatatypeProperty rdf:about="http://example.org/onto/prop/google_developer_connect_insights_config_app_hub_application">
    <rdfs:label>app_hub_application</rdfs:label>
    <rdfs:comment>The name of the App Hub Application.
Format:
projects/{project}/locations/{location}/applications/{application}</rdfs:comment>
    <rdfs:domain rdf:resource="http://example.org/onto/class/google_developer_connect_insights_config"/>
    <rdfs:range rdf:resource="http://www.w3.org/2001/XMLSchema#string"/>
  </owl:DatatypeProperty>
  <owl:DatatypeProperty rdf:about="http://example.org/onto/prop/google_developer_connect_insights_config_create_time">
    <rdfs:label>create_time</rdfs:label>
    <rdfs:comment>[Output only] Create timestamp</rdfs:comment>
    <rdfs:domain rdf:resource="http://example.org/onto/class/google_developer_connect_insights_config"/>
    <rdfs:range rdf:resource="http://www.w3.org/2001/XMLSchema#string"/>
  </owl:DatatypeProperty>
  <owl:DatatypeProperty rdf:about="http://example.org/onto/prop/google_developer_connect_insights_config_effective_annotations">
    <rdfs:label>effective_annotations</rdfs:label>
    <rdfs:comment>All of annotations (key/value pairs) present on the resource in GCP, including the annotations configured through Terraform, other clients and services.</rdfs:comment>
    <rdfs:domain rdf:resource="http://example.org/onto/class/google_developer_connect_insights_config"/>
    <rdfs:range rdf:resource="http://www.w3.org/2001/XMLSchema#string"/>
  </owl:DatatypeProperty>
  <owl:DatatypeProperty rdf:about="http://example.org/onto/prop/google_developer_connect_insights_config_effective_labels">
    <rdfs:label>effective_labels</rdfs:label>
    <rdfs:comment>All of labels (key/value pairs) present on the resource in GCP, including the labels configured through Terraform, other clients and services.</rdfs:comment>
    <rdfs:domain rdf:resource="http://example.org/onto/class/google_developer_connect_insights_config"/>
    <rdfs:range rdf:resource="http://www.w3.org/2001/XMLSchema#string"/>
  </owl:DatatypeProperty>
  <owl:DatatypeProperty rdf:about="http://example.org/onto/prop/google_developer_connect_insights_config_errors">
    <rdfs:label>errors</rdfs:label>
    <rdfs:comment>Any errors that occurred while setting up the InsightsConfig.
Each error will be in the format: 'field_name: error_message', e.g.
GetAppHubApplication: Permission denied while getting App Hub
application. Please grant permissions to the P4SA.</rdfs:comment>
    <rdfs:domain rdf:resource="http://example.org/onto/class/google_developer_connect_insights_config"/>
    <rdfs:range rdf:resource="http://www.w3.org/2001/XMLSchema#string"/>
  </owl:DatatypeProperty>
  <owl:DatatypeProperty rdf:about="http://example.org/onto/prop/google_developer_connect_insights_config_id">
    <rdfs:label>id</rdfs:label>
    <rdfs:domain rdf:resource="http://example.org/onto/class/google_developer_connect_insights_config"/>
    <rdfs:range rdf:resource="http://www.w3.org/2001/XMLSchema#string"/>
  </owl:DatatypeProperty>
  <owl:DatatypeProperty rdf:about="http://example.org/onto/prop/google_developer_connect_insights_config_insights_config_id">
    <rdfs:label>insights_config_id</rdfs:label>
    <rdfs:comment>ID of the requesting InsightsConfig.</rdfs:comment>
    <rdfs:domain rdf:resource="http://example.org/onto/class/google_developer_connect_insights_config"/>
    <rdfs:range rdf:resource="http://www.w3.org/2001/XMLSchema#string"/>
  </owl:DatatypeProperty>
  <owl:DatatypeProperty rdf:about="http://example.org/onto/prop/google_developer_connect_insights_config_labels">
    <rdfs:label>labels</rdfs:label>
    <rdfs:comment>Set of labels associated with an InsightsConfig.

**Note**: This field is non-authoritative, and will only manage the labels present in your configuration.
Please refer to the field 'effective_labels' for all of the labels present on the resource.</rdfs:comment>
    <rdfs:domain rdf:resource="http://example.org/onto/class/google_developer_connect_insights_config"/>
    <rdfs:range rdf:resource="http://www.w3.org/2001/XMLSchema#string"/>
  </owl:DatatypeProperty>
  <owl:DatatypeProperty rdf:about="http://example.org/onto/prop/google_developer_connect_insights_config_location">
    <rdfs:label>location</rdfs:label>
    <rdfs:comment>Resource ID segment making up resource 'name'. It identifies the resource within its parent collection as described in https://google.aip.dev/122.</rdfs:comment>
    <rdfs:domain rdf:resource="http://example.org/onto/class/google_developer_connect_insights_config"/>
    <rdfs:range rdf:resource="http://www.w3.org/2001/XMLSchema#string"/>
  </owl:DatatypeProperty>
  <owl:DatatypeProperty rdf:about="http://example.org/onto/prop/google_developer_connect_insights_config_name">
    <rdfs:label>name</rdfs:label>
    <rdfs:comment>Identifier. The name of the InsightsConfig.
Format:
projects/{project}/locations/{location}/insightsConfigs/{insightsConfig}</rdfs:comment>
    <rdfs:domain rdf:resource="http://example.org/onto/class/google_developer_connect_insights_config"/>
    <rdfs:range rdf:resource="http://www.w3.org/2001/XMLSchema#string"/>
  </owl:DatatypeProperty>
  <owl:DatatypeProperty rdf:about="http://example.org/onto/prop/google_developer_connect_insights_config_project">
    <rdfs:label>project</rdfs:label>
    <rdfs:domain rdf:resource="http://example.org/onto/class/google_developer_connect_insights_config"/>
    <rdfs:range rdf:resource="http://www.w3.org/2001/XMLSchema#string"/>
  </owl:DatatypeProperty>
  <owl:DatatypeProperty rdf:about="http://example.org/onto/prop/google_developer_connect_insights_config_reconciling">
    <rdfs:label>reconciling</rdfs:label>
    <rdfs:comment>Reconciling (https://google.aip.dev/128#reconciliation).
Set to true if the current state of InsightsConfig does not match the
user's intended state, and the service is actively updating the resource to
reconcile them. This can happen due to user-triggered updates or
system actions like failover or maintenance.</rdfs:comment>
    <rdfs:domain rdf:resource="http://example.org/onto/class/google_developer_connect_insights_config"/>
    <rdfs:range rdf:resource="http://www.w3.org/2001/XMLSchema#string"/>
  </owl:DatatypeProperty>
  <owl:DatatypeProperty rdf:about="http://example.org/onto/prop/google_developer_connect_insights_config_runtime_configs">
    <rdfs:label>runtime_configs</rdfs:label>
    <rdfs:comment>The runtime configurations where the application is deployed.</rdfs:comment>
    <rdfs:domain rdf:resource="http://example.org/onto/class/google_developer_connect_insights_config"/>
    <rdfs:range rdf:resource="http://www.w3.org/2001/XMLSchema#string"/>
  </owl:DatatypeProperty>
  <owl:DatatypeProperty rdf:about="http://example.org/onto/prop/google_developer_connect_insights_config_state">
    <rdfs:label>state</rdfs:label>
    <rdfs:comment>The state of the InsightsConfig.
Possible values:
STATE_UNSPECIFIED
PENDING
COMPLETE
ERROR</rdfs:comment>
    <rdfs:domain rdf:resource="http://example.org/onto/class/google_developer_connect_insights_config"/>
    <rdfs:range rdf:resource="http://www.w3.org/2001/XMLSchema#string"/>
  </owl:DatatypeProperty>
  <owl:DatatypeProperty rdf:about="http://example.org/onto/prop/google_developer_connect_insights_config_terraform_labels">
    <rdfs:label>terraform_labels</rdfs:label>
    <rdfs:comment>The combination of labels configured directly on the resource
 and default labels configured on the provider.</rdfs:comment>
    <rdfs:domain rdf:resource="http://example.org/onto/class/google_developer_connect_insights_config"/>
    <rdfs:range rdf:resource="http://www.w3.org/2001/XMLSchema#string"/>
  </owl:DatatypeProperty>
  <owl:DatatypeProperty rdf:about="http://example.org/onto/prop/google_developer_connect_insights_config_update_time">
    <rdfs:label>update_time</rdfs:label>
    <rdfs:comment>[Output only] Update timestamp</rdfs:comment>
    <rdfs:domain rdf:resource="http://example.org/onto/class/google_developer_connect_insights_config"/>
    <rdfs:range rdf:resource="http://www.w3.org/2001/XMLSchema#string"/>
  </owl:DatatypeProperty>
  <owl:DatatypeProperty rdf:about="http://example.org/onto/prop/google_developer_connect_insights_config_uri">
    <rdfs:label>uri</rdfs:label>
    <rdfs:comment>The URI of the artifact that is deployed.
e.g. 'us-docker.pkg.dev/my-project/my-repo/image'.
The URI does not include the tag / digest because it captures a lineage of
artifacts.</rdfs:comment>
    <rdfs:domain rdf:resource="http://example.org/onto/class/google_developer_connect_insights_config"/>
    <rdfs:range rdf:resource="http://www.w3.org/2001/XMLSchema#string"/>
  </owl:DatatypeProperty>
  <owl:DatatypeProperty rdf:about="http://example.org/onto/prop/google_developer_connect_insights_config_project_id">
    <rdfs:label>project_id</rdfs:label>
    <rdfs:comment>The project id of the project where the provenance is stored.</rdfs:comment>
    <rdfs:domain rdf:resource="http://example.org/onto/class/google_developer_connect_insights_config"/>
    <rdfs:range rdf:resource="http://www.w3.org/2001/XMLSchema#string"/>
  </owl:DatatypeProperty>
  <owl:DatatypeProperty rdf:about="http://example.org/onto/prop/google_developer_connect_insights_config_artifact_registry_package">
    <rdfs:label>artifact_registry_package</rdfs:label>
    <rdfs:comment>The name of the artifact registry package.</rdfs:comment>
    <rdfs:domain rdf:resource="http://example.org/onto/class/google_developer_connect_insights_config"/>
    <rdfs:range rdf:resource="http://www.w3.org/2001/XMLSchema#string"/>
  </owl:DatatypeProperty>
  <owl:DatatypeProperty rdf:about="http://example.org/onto/prop/google_developer_connect_insights_config_project_id">
    <rdfs:label>project_id</rdfs:label>
    <rdfs:comment>The host project of Artifact Registry.</rdfs:comment>
    <rdfs:domain rdf:resource="http://example.org/onto/class/google_developer_connect_insights_config"/>
    <rdfs:range rdf:resource="http://www.w3.org/2001/XMLSchema#string"/>
  </owl:DatatypeProperty>
  <owl:DatatypeProperty rdf:about="http://example.org/onto/prop/google_developer_connect_insights_config_create">
    <rdfs:label>create</rdfs:label>
    <rdfs:domain rdf:resource="http://example.org/onto/class/google_developer_connect_insights_config"/>
    <rdfs:range rdf:resource="http://www.w3.org/2001/XMLSchema#string"/>
  </owl:DatatypeProperty>
  <owl:DatatypeProperty rdf:about="http://example.org/onto/prop/google_developer_connect_insights_config_delete">
    <rdfs:label>delete</rdfs:label>
    <rdfs:domain rdf:resource="http://example.org/onto/class/google_developer_connect_insights_config"/>
    <rdfs:range rdf:resource="http://www.w3.org/2001/XMLSchema#string"/>
  </owl:DatatypeProperty>
  <owl:DatatypeProperty rdf:about="http://example.org/onto/prop/google_developer_connect_insights_config_update">
    <rdfs:label>update</rdfs:label>
    <rdfs:domain rdf:resource="http://example.org/onto/class/google_developer_connect_insights_config"/>
    <rdfs:range rdf:resource="http://www.w3.org/2001/XMLSchema#string"/>
  </owl:DatatypeProperty>
</rdf:RDF>
