<?xml version="1.0" encoding="UTF-8"?>
<rdf:RDF
  xmlns:rdf="http://www.w3.org/1999/02/22-rdf-syntax-ns#"
  xmlns:rdfs="http://www.w3.org/2000/01/rdf-schema#"
  xmlns:owl="http://www.w3.org/2002/07/owl#"
  xmlns:xsd="http://www.w3.org/2001/XMLSchema#"
  xml:base="http://example.org/onto/">
  <owl:Class rdf:about="http://example.org/onto/class/google_compute_router_interface">
    <rdfs:label>google_compute_router_interface</rdfs:label>
    <rdfs:comment>#
#     ***     AUTO GENERATED CODE    ***    Type: Handwritten     ***
#
# ----------------------------------------------------------------------------
#
#     This code is generated by Magic Modules using the following:
#
#     Source file: https://github.com/GoogleCloudPlatform/magic-modules/tree/main/mmv1/third_party/terraform/website/docs/r/compute_router_interface.html.markdown
#
#     DO NOT EDIT this file directly. Any changes made to this file will be
#     overwritten during the next generation cycle.
#
# ----------------------------------------------------------------------------
subcategory: "Compute Engine"
description: |-
  Manages a Cloud Router interface.
---</rdfs:comment>
  </owl:Class>
  <owl:DatatypeProperty rdf:about="http://example.org/onto/prop/google_compute_router_interface_id">
    <rdfs:label>id</rdfs:label>
    <rdfs:domain rdf:resource="http://example.org/onto/class/google_compute_router_interface"/>
    <rdfs:range rdf:resource="http://www.w3.org/2001/XMLSchema#string"/>
  </owl:DatatypeProperty>
  <owl:DatatypeProperty rdf:about="http://example.org/onto/prop/google_compute_router_interface_interconnect_attachment">
    <rdfs:label>interconnect_attachment</rdfs:label>
    <rdfs:comment>The name or resource link to the VLAN interconnect for this interface. Changing this forces a new interface to be created. Only one of interconnect_attachment, subnetwork or vpn_tunnel can be specified.</rdfs:comment>
    <rdfs:domain rdf:resource="http://example.org/onto/class/google_compute_router_interface"/>
    <rdfs:range rdf:resource="http://www.w3.org/2001/XMLSchema#string"/>
  </owl:DatatypeProperty>
  <owl:DatatypeProperty rdf:about="http://example.org/onto/prop/google_compute_router_interface_ip_range">
    <rdfs:label>ip_range</rdfs:label>
    <rdfs:comment>The IP address and range of the interface. The IP range must be in the RFC3927 link-local IP space. Changing this forces a new interface to be created.</rdfs:comment>
    <rdfs:domain rdf:resource="http://example.org/onto/class/google_compute_router_interface"/>
    <rdfs:range rdf:resource="http://www.w3.org/2001/XMLSchema#string"/>
  </owl:DatatypeProperty>
  <owl:DatatypeProperty rdf:about="http://example.org/onto/prop/google_compute_router_interface_ip_version">
    <rdfs:label>ip_version</rdfs:label>
    <rdfs:comment>IP version of this interface.</rdfs:comment>
    <rdfs:domain rdf:resource="http://example.org/onto/class/google_compute_router_interface"/>
    <rdfs:range rdf:resource="http://www.w3.org/2001/XMLSchema#string"/>
  </owl:DatatypeProperty>
  <owl:DatatypeProperty rdf:about="http://example.org/onto/prop/google_compute_router_interface_name">
    <rdfs:label>name</rdfs:label>
    <rdfs:comment>A unique name for the interface, required by GCE. Changing this forces a new interface to be created.</rdfs:comment>
    <rdfs:domain rdf:resource="http://example.org/onto/class/google_compute_router_interface"/>
    <rdfs:range rdf:resource="http://www.w3.org/2001/XMLSchema#string"/>
  </owl:DatatypeProperty>
  <owl:DatatypeProperty rdf:about="http://example.org/onto/prop/google_compute_router_interface_private_ip_address">
    <rdfs:label>private_ip_address</rdfs:label>
    <rdfs:comment>The regional private internal IP address that is used to establish BGP sessions to a VM instance acting as a third-party Router Appliance. Changing this forces a new interface to be created.</rdfs:comment>
    <rdfs:domain rdf:resource="http://example.org/onto/class/google_compute_router_interface"/>
    <rdfs:range rdf:resource="http://www.w3.org/2001/XMLSchema#string"/>
  </owl:DatatypeProperty>
  <owl:DatatypeProperty rdf:about="http://example.org/onto/prop/google_compute_router_interface_project">
    <rdfs:label>project</rdfs:label>
    <rdfs:comment>The ID of the project in which this interface's router belongs. If it is not provided, the provider project is used. Changing this forces a new interface to be created.</rdfs:comment>
    <rdfs:domain rdf:resource="http://example.org/onto/class/google_compute_router_interface"/>
    <rdfs:range rdf:resource="http://www.w3.org/2001/XMLSchema#string"/>
  </owl:DatatypeProperty>
  <owl:DatatypeProperty rdf:about="http://example.org/onto/prop/google_compute_router_interface_redundant_interface">
    <rdfs:label>redundant_interface</rdfs:label>
    <rdfs:comment>The name of the interface that is redundant to this interface. Changing this forces a new interface to be created.</rdfs:comment>
    <rdfs:domain rdf:resource="http://example.org/onto/class/google_compute_router_interface"/>
    <rdfs:range rdf:resource="http://www.w3.org/2001/XMLSchema#string"/>
  </owl:DatatypeProperty>
  <owl:DatatypeProperty rdf:about="http://example.org/onto/prop/google_compute_router_interface_region">
    <rdfs:label>region</rdfs:label>
    <rdfs:comment>The region this interface's router sits in. If not specified, the project region will be used. Changing this forces a new interface to be created.</rdfs:comment>
    <rdfs:domain rdf:resource="http://example.org/onto/class/google_compute_router_interface"/>
    <rdfs:range rdf:resource="http://www.w3.org/2001/XMLSchema#string"/>
  </owl:DatatypeProperty>
  <owl:DatatypeProperty rdf:about="http://example.org/onto/prop/google_compute_router_interface_router">
    <rdfs:label>router</rdfs:label>
    <rdfs:comment>The name of the router this interface will be attached to. Changing this forces a new interface to be created.</rdfs:comment>
    <rdfs:domain rdf:resource="http://example.org/onto/class/google_compute_router_interface"/>
    <rdfs:range rdf:resource="http://www.w3.org/2001/XMLSchema#string"/>
  </owl:DatatypeProperty>
  <owl:DatatypeProperty rdf:about="http://example.org/onto/prop/google_compute_router_interface_subnetwork">
    <rdfs:label>subnetwork</rdfs:label>
    <rdfs:comment>The URI of the subnetwork resource that this interface belongs to, which must be in the same region as the Cloud Router. Changing this forces a new interface to be created. Only one of subnetwork, interconnect_attachment or vpn_tunnel can be specified.</rdfs:comment>
    <rdfs:domain rdf:resource="http://example.org/onto/class/google_compute_router_interface"/>
    <rdfs:range rdf:resource="http://www.w3.org/2001/XMLSchema#string"/>
  </owl:DatatypeProperty>
  <owl:DatatypeProperty rdf:about="http://example.org/onto/prop/google_compute_router_interface_vpn_tunnel">
    <rdfs:label>vpn_tunnel</rdfs:label>
    <rdfs:comment>The name or resource link to the VPN tunnel this interface will be linked to. Changing this forces a new interface to be created. Only one of vpn_tunnel, interconnect_attachment or subnetwork can be specified.</rdfs:comment>
    <rdfs:domain rdf:resource="http://example.org/onto/class/google_compute_router_interface"/>
    <rdfs:range rdf:resource="http://www.w3.org/2001/XMLSchema#string"/>
  </owl:DatatypeProperty>
  <owl:DatatypeProperty rdf:about="http://example.org/onto/prop/google_compute_router_interface_create">
    <rdfs:label>create</rdfs:label>
    <rdfs:domain rdf:resource="http://example.org/onto/class/google_compute_router_interface"/>
    <rdfs:range rdf:resource="http://www.w3.org/2001/XMLSchema#string"/>
  </owl:DatatypeProperty>
  <owl:DatatypeProperty rdf:about="http://example.org/onto/prop/google_compute_router_interface_delete">
    <rdfs:label>delete</rdfs:label>
    <rdfs:domain rdf:resource="http://example.org/onto/class/google_compute_router_interface"/>
    <rdfs:range rdf:resource="http://www.w3.org/2001/XMLSchema#string"/>
  </owl:DatatypeProperty>
</rdf:RDF>
