<?xml version="1.0" encoding="UTF-8"?>
<rdf:RDF
  xmlns:rdf="http://www.w3.org/1999/02/22-rdf-syntax-ns#"
  xmlns:rdfs="http://www.w3.org/2000/01/rdf-schema#"
  xmlns:owl="http://www.w3.org/2002/07/owl#"
  xmlns:xsd="http://www.w3.org/2001/XMLSchema#"
  xml:base="http://example.org/onto/">
  <owl:Class rdf:about="http://example.org/onto/class/google_dialogflow_intent">
    <rdfs:label>google_dialogflow_intent</rdfs:label>
    <rdfs:comment>#
#     ***     AUTO GENERATED CODE    ***    Type: MMv1     ***
#
# ----------------------------------------------------------------------------
#
#     This code is generated by Magic Modules using the following:
#
#     Configuration: https:#github.com/GoogleCloudPlatform/magic-modules/tree/main/mmv1/products/dialogflow/Intent.yaml
#     Template:      https:#github.com/GoogleCloudPlatform/magic-modules/tree/main/mmv1/templates/terraform/resource.html.markdown.tmpl
#
#     DO NOT EDIT this file directly. Any changes made to this file will be
#     overwritten during the next generation cycle.
#
# ----------------------------------------------------------------------------
subcategory: "Dialogflow"
description: |-
  Represents a Dialogflow intent.
---</rdfs:comment>
  </owl:Class>
  <owl:DatatypeProperty rdf:about="http://example.org/onto/prop/google_dialogflow_intent_action">
    <rdfs:label>action</rdfs:label>
    <rdfs:comment>The name of the action associated with the intent.
Note: The action name must not contain whitespaces.</rdfs:comment>
    <rdfs:domain rdf:resource="http://example.org/onto/class/google_dialogflow_intent"/>
    <rdfs:range rdf:resource="http://www.w3.org/2001/XMLSchema#string"/>
  </owl:DatatypeProperty>
  <owl:DatatypeProperty rdf:about="http://example.org/onto/prop/google_dialogflow_intent_default_response_platforms">
    <rdfs:label>default_response_platforms</rdfs:label>
    <rdfs:comment>The list of platforms for which the first responses will be copied from the messages in PLATFORM_UNSPECIFIED
(i.e. default platform). Possible values: ["FACEBOOK", "SLACK", "TELEGRAM", "KIK", "SKYPE", "LINE", "VIBER", "ACTIONS_ON_GOOGLE", "GOOGLE_HANGOUTS"]</rdfs:comment>
    <rdfs:domain rdf:resource="http://example.org/onto/class/google_dialogflow_intent"/>
    <rdfs:range rdf:resource="http://www.w3.org/2001/XMLSchema#string"/>
  </owl:DatatypeProperty>
  <owl:DatatypeProperty rdf:about="http://example.org/onto/prop/google_dialogflow_intent_display_name">
    <rdfs:label>display_name</rdfs:label>
    <rdfs:comment>The name of this intent to be displayed on the console.</rdfs:comment>
    <rdfs:domain rdf:resource="http://example.org/onto/class/google_dialogflow_intent"/>
    <rdfs:range rdf:resource="http://www.w3.org/2001/XMLSchema#string"/>
  </owl:DatatypeProperty>
  <owl:DatatypeProperty rdf:about="http://example.org/onto/prop/google_dialogflow_intent_events">
    <rdfs:label>events</rdfs:label>
    <rdfs:comment>The collection of event names that trigger the intent. If the collection of input contexts is not empty, all of
the contexts must be present in the active user session for an event to trigger this intent. See the
[events reference](https://cloud.google.com/dialogflow/docs/events-overview) for more details.</rdfs:comment>
    <rdfs:domain rdf:resource="http://example.org/onto/class/google_dialogflow_intent"/>
    <rdfs:range rdf:resource="http://www.w3.org/2001/XMLSchema#string"/>
  </owl:DatatypeProperty>
  <owl:DatatypeProperty rdf:about="http://example.org/onto/prop/google_dialogflow_intent_followup_intent_info">
    <rdfs:label>followup_intent_info</rdfs:label>
    <rdfs:comment>Information about all followup intents that have this intent as a direct or indirect parent. We populate this field
only in the output.</rdfs:comment>
    <rdfs:domain rdf:resource="http://example.org/onto/class/google_dialogflow_intent"/>
    <rdfs:range rdf:resource="http://www.w3.org/2001/XMLSchema#string"/>
  </owl:DatatypeProperty>
  <owl:DatatypeProperty rdf:about="http://example.org/onto/prop/google_dialogflow_intent_id">
    <rdfs:label>id</rdfs:label>
    <rdfs:domain rdf:resource="http://example.org/onto/class/google_dialogflow_intent"/>
    <rdfs:range rdf:resource="http://www.w3.org/2001/XMLSchema#string"/>
  </owl:DatatypeProperty>
  <owl:DatatypeProperty rdf:about="http://example.org/onto/prop/google_dialogflow_intent_input_context_names">
    <rdfs:label>input_context_names</rdfs:label>
    <rdfs:comment>The list of context names required for this intent to be triggered.
Format: projects/<Project ID>/agent/sessions/-/contexts/<Context ID>.</rdfs:comment>
    <rdfs:domain rdf:resource="http://example.org/onto/class/google_dialogflow_intent"/>
    <rdfs:range rdf:resource="http://www.w3.org/2001/XMLSchema#string"/>
  </owl:DatatypeProperty>
  <owl:DatatypeProperty rdf:about="http://example.org/onto/prop/google_dialogflow_intent_is_fallback">
    <rdfs:label>is_fallback</rdfs:label>
    <rdfs:comment>Indicates whether this is a fallback intent.</rdfs:comment>
    <rdfs:domain rdf:resource="http://example.org/onto/class/google_dialogflow_intent"/>
    <rdfs:range rdf:resource="http://www.w3.org/2001/XMLSchema#string"/>
  </owl:DatatypeProperty>
  <owl:DatatypeProperty rdf:about="http://example.org/onto/prop/google_dialogflow_intent_ml_disabled">
    <rdfs:label>ml_disabled</rdfs:label>
    <rdfs:comment>Indicates whether Machine Learning is disabled for the intent.
Note: If mlDisabled setting is set to true, then this intent is not taken into account during inference in ML
ONLY match mode. Also, auto-markup in the UI is turned off.</rdfs:comment>
    <rdfs:domain rdf:resource="http://example.org/onto/class/google_dialogflow_intent"/>
    <rdfs:range rdf:resource="http://www.w3.org/2001/XMLSchema#string"/>
  </owl:DatatypeProperty>
  <owl:DatatypeProperty rdf:about="http://example.org/onto/prop/google_dialogflow_intent_name">
    <rdfs:label>name</rdfs:label>
    <rdfs:comment>The unique identifier of this intent.
Format: projects/<Project ID>/agent/intents/<Intent ID>.</rdfs:comment>
    <rdfs:domain rdf:resource="http://example.org/onto/class/google_dialogflow_intent"/>
    <rdfs:range rdf:resource="http://www.w3.org/2001/XMLSchema#string"/>
  </owl:DatatypeProperty>
  <owl:DatatypeProperty rdf:about="http://example.org/onto/prop/google_dialogflow_intent_parent_followup_intent_name">
    <rdfs:label>parent_followup_intent_name</rdfs:label>
    <rdfs:comment>The unique identifier of the parent intent in the chain of followup intents.
Format: projects/<Project ID>/agent/intents/<Intent ID>.</rdfs:comment>
    <rdfs:domain rdf:resource="http://example.org/onto/class/google_dialogflow_intent"/>
    <rdfs:range rdf:resource="http://www.w3.org/2001/XMLSchema#string"/>
  </owl:DatatypeProperty>
  <owl:DatatypeProperty rdf:about="http://example.org/onto/prop/google_dialogflow_intent_priority">
    <rdfs:label>priority</rdfs:label>
    <rdfs:comment>The priority of this intent. Higher numbers represent higher priorities.
  - If the supplied value is unspecified or 0, the service translates the value to 500,000, which corresponds
  to the Normal priority in the console.
  - If the supplied value is negative, the intent is ignored in runtime detect intent requests.</rdfs:comment>
    <rdfs:domain rdf:resource="http://example.org/onto/class/google_dialogflow_intent"/>
    <rdfs:range rdf:resource="http://www.w3.org/2001/XMLSchema#string"/>
  </owl:DatatypeProperty>
  <owl:DatatypeProperty rdf:about="http://example.org/onto/prop/google_dialogflow_intent_project">
    <rdfs:label>project</rdfs:label>
    <rdfs:domain rdf:resource="http://example.org/onto/class/google_dialogflow_intent"/>
    <rdfs:range rdf:resource="http://www.w3.org/2001/XMLSchema#string"/>
  </owl:DatatypeProperty>
  <owl:DatatypeProperty rdf:about="http://example.org/onto/prop/google_dialogflow_intent_reset_contexts">
    <rdfs:label>reset_contexts</rdfs:label>
    <rdfs:comment>Indicates whether to delete all contexts in the current session when this intent is matched.</rdfs:comment>
    <rdfs:domain rdf:resource="http://example.org/onto/class/google_dialogflow_intent"/>
    <rdfs:range rdf:resource="http://www.w3.org/2001/XMLSchema#string"/>
  </owl:DatatypeProperty>
  <owl:DatatypeProperty rdf:about="http://example.org/onto/prop/google_dialogflow_intent_root_followup_intent_name">
    <rdfs:label>root_followup_intent_name</rdfs:label>
    <rdfs:comment>The unique identifier of the root intent in the chain of followup intents. It identifies the correct followup
intents chain for this intent.
Format: projects/<Project ID>/agent/intents/<Intent ID>.</rdfs:comment>
    <rdfs:domain rdf:resource="http://example.org/onto/class/google_dialogflow_intent"/>
    <rdfs:range rdf:resource="http://www.w3.org/2001/XMLSchema#string"/>
  </owl:DatatypeProperty>
  <owl:DatatypeProperty rdf:about="http://example.org/onto/prop/google_dialogflow_intent_webhook_state">
    <rdfs:label>webhook_state</rdfs:label>
    <rdfs:comment>Indicates whether webhooks are enabled for the intent.
* WEBHOOK_STATE_ENABLED: Webhook is enabled in the agent and in the intent.
* WEBHOOK_STATE_ENABLED_FOR_SLOT_FILLING: Webhook is enabled in the agent and in the intent. Also, each slot
filling prompt is forwarded to the webhook. Possible values: ["WEBHOOK_STATE_ENABLED", "WEBHOOK_STATE_ENABLED_FOR_SLOT_FILLING"]</rdfs:comment>
    <rdfs:domain rdf:resource="http://example.org/onto/class/google_dialogflow_intent"/>
    <rdfs:range rdf:resource="http://www.w3.org/2001/XMLSchema#string"/>
  </owl:DatatypeProperty>
  <owl:DatatypeProperty rdf:about="http://example.org/onto/prop/google_dialogflow_intent_create">
    <rdfs:label>create</rdfs:label>
    <rdfs:domain rdf:resource="http://example.org/onto/class/google_dialogflow_intent"/>
    <rdfs:range rdf:resource="http://www.w3.org/2001/XMLSchema#string"/>
  </owl:DatatypeProperty>
  <owl:DatatypeProperty rdf:about="http://example.org/onto/prop/google_dialogflow_intent_delete">
    <rdfs:label>delete</rdfs:label>
    <rdfs:domain rdf:resource="http://example.org/onto/class/google_dialogflow_intent"/>
    <rdfs:range rdf:resource="http://www.w3.org/2001/XMLSchema#string"/>
  </owl:DatatypeProperty>
  <owl:DatatypeProperty rdf:about="http://example.org/onto/prop/google_dialogflow_intent_update">
    <rdfs:label>update</rdfs:label>
    <rdfs:domain rdf:resource="http://example.org/onto/class/google_dialogflow_intent"/>
    <rdfs:range rdf:resource="http://www.w3.org/2001/XMLSchema#string"/>
  </owl:DatatypeProperty>
</rdf:RDF>
