<?xml version="1.0" encoding="UTF-8"?>
<rdf:RDF
  xmlns:rdf="http://www.w3.org/1999/02/22-rdf-syntax-ns#"
  xmlns:rdfs="http://www.w3.org/2000/01/rdf-schema#"
  xmlns:owl="http://www.w3.org/2002/07/owl#"
  xmlns:xsd="http://www.w3.org/2001/XMLSchema#"
  xml:base="http://example.org/onto/">
  <owl:Class rdf:about="http://example.org/onto/class/google_monitoring_slo">
    <rdfs:label>google_monitoring_slo</rdfs:label>
    <rdfs:comment>#
#     ***     AUTO GENERATED CODE    ***    Type: MMv1     ***
#
# ----------------------------------------------------------------------------
#
#     This code is generated by Magic Modules using the following:
#
#     Configuration: https:#github.com/GoogleCloudPlatform/magic-modules/tree/main/mmv1/products/monitoring/Slo.yaml
#     Template:      https:#github.com/GoogleCloudPlatform/magic-modules/tree/main/mmv1/templates/terraform/resource.html.markdown.tmpl
#
#     DO NOT EDIT this file directly. Any changes made to this file will be
#     overwritten during the next generation cycle.
#
# ----------------------------------------------------------------------------
subcategory: "Cloud (Stackdriver) Monitoring"
description: |-
  A Service-Level Objective (SLO) describes the level of desired good
  service.
---</rdfs:comment>
  </owl:Class>
  <owl:DatatypeProperty rdf:about="http://example.org/onto/prop/google_monitoring_slo_calendar_period">
    <rdfs:label>calendar_period</rdfs:label>
    <rdfs:comment>A calendar period, semantically "since the start of the current
<calendarPeriod>". Possible values: ["DAY", "WEEK", "FORTNIGHT", "MONTH"]</rdfs:comment>
    <rdfs:domain rdf:resource="http://example.org/onto/class/google_monitoring_slo"/>
    <rdfs:range rdf:resource="http://www.w3.org/2001/XMLSchema#string"/>
  </owl:DatatypeProperty>
  <owl:DatatypeProperty rdf:about="http://example.org/onto/prop/google_monitoring_slo_display_name">
    <rdfs:label>display_name</rdfs:label>
    <rdfs:comment>Name used for UI elements listing this SLO.</rdfs:comment>
    <rdfs:domain rdf:resource="http://example.org/onto/class/google_monitoring_slo"/>
    <rdfs:range rdf:resource="http://www.w3.org/2001/XMLSchema#string"/>
  </owl:DatatypeProperty>
  <owl:DatatypeProperty rdf:about="http://example.org/onto/prop/google_monitoring_slo_goal">
    <rdfs:label>goal</rdfs:label>
    <rdfs:comment>The fraction of service that must be good in order for this objective
to be met. 0 < goal <= 0.999</rdfs:comment>
    <rdfs:domain rdf:resource="http://example.org/onto/class/google_monitoring_slo"/>
    <rdfs:range rdf:resource="http://www.w3.org/2001/XMLSchema#string"/>
  </owl:DatatypeProperty>
  <owl:DatatypeProperty rdf:about="http://example.org/onto/prop/google_monitoring_slo_id">
    <rdfs:label>id</rdfs:label>
    <rdfs:domain rdf:resource="http://example.org/onto/class/google_monitoring_slo"/>
    <rdfs:range rdf:resource="http://www.w3.org/2001/XMLSchema#string"/>
  </owl:DatatypeProperty>
  <owl:DatatypeProperty rdf:about="http://example.org/onto/prop/google_monitoring_slo_name">
    <rdfs:label>name</rdfs:label>
    <rdfs:comment>The full resource name for this service. The syntax is:
projects/[PROJECT_ID_OR_NUMBER]/services/[SERVICE_ID]/serviceLevelObjectives/[SLO_NAME]</rdfs:comment>
    <rdfs:domain rdf:resource="http://example.org/onto/class/google_monitoring_slo"/>
    <rdfs:range rdf:resource="http://www.w3.org/2001/XMLSchema#string"/>
  </owl:DatatypeProperty>
  <owl:DatatypeProperty rdf:about="http://example.org/onto/prop/google_monitoring_slo_project">
    <rdfs:label>project</rdfs:label>
    <rdfs:domain rdf:resource="http://example.org/onto/class/google_monitoring_slo"/>
    <rdfs:range rdf:resource="http://www.w3.org/2001/XMLSchema#string"/>
  </owl:DatatypeProperty>
  <owl:DatatypeProperty rdf:about="http://example.org/onto/prop/google_monitoring_slo_rolling_period_days">
    <rdfs:label>rolling_period_days</rdfs:label>
    <rdfs:comment>A rolling time period, semantically "in the past X days".
Must be between 1 to 30 days, inclusive.</rdfs:comment>
    <rdfs:domain rdf:resource="http://example.org/onto/class/google_monitoring_slo"/>
    <rdfs:range rdf:resource="http://www.w3.org/2001/XMLSchema#string"/>
  </owl:DatatypeProperty>
  <owl:DatatypeProperty rdf:about="http://example.org/onto/prop/google_monitoring_slo_service">
    <rdfs:label>service</rdfs:label>
    <rdfs:comment>ID of the service to which this SLO belongs.</rdfs:comment>
    <rdfs:domain rdf:resource="http://example.org/onto/class/google_monitoring_slo"/>
    <rdfs:range rdf:resource="http://www.w3.org/2001/XMLSchema#string"/>
  </owl:DatatypeProperty>
  <owl:DatatypeProperty rdf:about="http://example.org/onto/prop/google_monitoring_slo_slo_id">
    <rdfs:label>slo_id</rdfs:label>
    <rdfs:comment>The id to use for this ServiceLevelObjective. If omitted, an id will be generated instead.</rdfs:comment>
    <rdfs:domain rdf:resource="http://example.org/onto/class/google_monitoring_slo"/>
    <rdfs:range rdf:resource="http://www.w3.org/2001/XMLSchema#string"/>
  </owl:DatatypeProperty>
  <owl:DatatypeProperty rdf:about="http://example.org/onto/prop/google_monitoring_slo_user_labels">
    <rdfs:label>user_labels</rdfs:label>
    <rdfs:comment>This field is intended to be used for organizing and identifying the AlertPolicy
objects.The field can contain up to 64 entries. Each key and value is limited
to 63 Unicode characters or 128 bytes, whichever is smaller. Labels and values
can contain only lowercase letters, numerals, underscores, and dashes. Keys
must begin with a letter.</rdfs:comment>
    <rdfs:domain rdf:resource="http://example.org/onto/class/google_monitoring_slo"/>
    <rdfs:range rdf:resource="http://www.w3.org/2001/XMLSchema#string"/>
  </owl:DatatypeProperty>
  <owl:DatatypeProperty rdf:about="http://example.org/onto/prop/google_monitoring_slo_location">
    <rdfs:label>location</rdfs:label>
    <rdfs:comment>An optional set of locations to which this SLI is relevant.
Telemetry from other locations will not be used to calculate
performance for this SLI. If omitted, this SLI applies to all
locations in which the Service has activity. For service types
that don't support breaking down by location, setting this
field will result in an error.</rdfs:comment>
    <rdfs:domain rdf:resource="http://example.org/onto/class/google_monitoring_slo"/>
    <rdfs:range rdf:resource="http://www.w3.org/2001/XMLSchema#string"/>
  </owl:DatatypeProperty>
  <owl:DatatypeProperty rdf:about="http://example.org/onto/prop/google_monitoring_slo_method">
    <rdfs:label>method</rdfs:label>
    <rdfs:comment>An optional set of RPCs to which this SLI is relevant.
Telemetry from other methods will not be used to calculate
performance for this SLI. If omitted, this SLI applies to all
the Service's methods. For service types that don't support
breaking down by method, setting this field will result in an
error.</rdfs:comment>
    <rdfs:domain rdf:resource="http://example.org/onto/class/google_monitoring_slo"/>
    <rdfs:range rdf:resource="http://www.w3.org/2001/XMLSchema#string"/>
  </owl:DatatypeProperty>
  <owl:DatatypeProperty rdf:about="http://example.org/onto/prop/google_monitoring_slo_version">
    <rdfs:label>version</rdfs:label>
    <rdfs:comment>The set of API versions to which this SLI is relevant.
Telemetry from other API versions will not be used to
calculate performance for this SLI. If omitted,
this SLI applies to all API versions. For service types
that don't support breaking down by version, setting this
field will result in an error.</rdfs:comment>
    <rdfs:domain rdf:resource="http://example.org/onto/class/google_monitoring_slo"/>
    <rdfs:range rdf:resource="http://www.w3.org/2001/XMLSchema#string"/>
  </owl:DatatypeProperty>
  <owl:DatatypeProperty rdf:about="http://example.org/onto/prop/google_monitoring_slo_enabled">
    <rdfs:label>enabled</rdfs:label>
    <rdfs:comment>Whether an availability SLI is enabled or not. Must be set to true. Defaults to 'true'.</rdfs:comment>
    <rdfs:domain rdf:resource="http://example.org/onto/class/google_monitoring_slo"/>
    <rdfs:range rdf:resource="http://www.w3.org/2001/XMLSchema#string"/>
  </owl:DatatypeProperty>
  <owl:DatatypeProperty rdf:about="http://example.org/onto/prop/google_monitoring_slo_threshold">
    <rdfs:label>threshold</rdfs:label>
    <rdfs:comment>A duration string, e.g. 10s.
Good service is defined to be the count of requests made to
this service that return in no more than threshold.</rdfs:comment>
    <rdfs:domain rdf:resource="http://example.org/onto/class/google_monitoring_slo"/>
    <rdfs:range rdf:resource="http://www.w3.org/2001/XMLSchema#string"/>
  </owl:DatatypeProperty>
  <owl:DatatypeProperty rdf:about="http://example.org/onto/prop/google_monitoring_slo_distribution_filter">
    <rdfs:label>distribution_filter</rdfs:label>
    <rdfs:comment>A TimeSeries [monitoring filter](https://cloud.google.com/monitoring/api/v3/filters)
aggregating values to quantify the good service provided.

Must have ValueType = DISTRIBUTION and
MetricKind = DELTA or MetricKind = CUMULATIVE.</rdfs:comment>
    <rdfs:domain rdf:resource="http://example.org/onto/class/google_monitoring_slo"/>
    <rdfs:range rdf:resource="http://www.w3.org/2001/XMLSchema#string"/>
  </owl:DatatypeProperty>
  <owl:DatatypeProperty rdf:about="http://example.org/onto/prop/google_monitoring_slo_max">
    <rdfs:label>max</rdfs:label>
    <rdfs:comment>max value for the range (inclusive). If not given,
will be set to 0</rdfs:comment>
    <rdfs:domain rdf:resource="http://example.org/onto/class/google_monitoring_slo"/>
    <rdfs:range rdf:resource="http://www.w3.org/2001/XMLSchema#string"/>
  </owl:DatatypeProperty>
  <owl:DatatypeProperty rdf:about="http://example.org/onto/prop/google_monitoring_slo_min">
    <rdfs:label>min</rdfs:label>
    <rdfs:comment>Min value for the range (inclusive). If not given,
will be set to 0</rdfs:comment>
    <rdfs:domain rdf:resource="http://example.org/onto/class/google_monitoring_slo"/>
    <rdfs:range rdf:resource="http://www.w3.org/2001/XMLSchema#string"/>
  </owl:DatatypeProperty>
  <owl:DatatypeProperty rdf:about="http://example.org/onto/prop/google_monitoring_slo_bad_service_filter">
    <rdfs:label>bad_service_filter</rdfs:label>
    <rdfs:comment>A TimeSeries [monitoring filter](https://cloud.google.com/monitoring/api/v3/filters)
quantifying bad service provided, either demanded service that
was not provided or demanded service that was of inadequate
quality.

Must have ValueType = DOUBLE or ValueType = INT64 and
must have MetricKind = DELTA or MetricKind = CUMULATIVE.

Exactly two of 'good_service_filter','bad_service_filter','total_service_filter'
must be set (good + bad = total is assumed).</rdfs:comment>
    <rdfs:domain rdf:resource="http://example.org/onto/class/google_monitoring_slo"/>
    <rdfs:range rdf:resource="http://www.w3.org/2001/XMLSchema#string"/>
  </owl:DatatypeProperty>
  <owl:DatatypeProperty rdf:about="http://example.org/onto/prop/google_monitoring_slo_good_service_filter">
    <rdfs:label>good_service_filter</rdfs:label>
    <rdfs:comment>A TimeSeries [monitoring filter](https://cloud.google.com/monitoring/api/v3/filters)
quantifying good service provided.
Must have ValueType = DOUBLE or ValueType = INT64 and
must have MetricKind = DELTA or MetricKind = CUMULATIVE.

Exactly two of 'good_service_filter','bad_service_filter','total_service_filter'
must be set (good + bad = total is assumed).</rdfs:comment>
    <rdfs:domain rdf:resource="http://example.org/onto/class/google_monitoring_slo"/>
    <rdfs:range rdf:resource="http://www.w3.org/2001/XMLSchema#string"/>
  </owl:DatatypeProperty>
  <owl:DatatypeProperty rdf:about="http://example.org/onto/prop/google_monitoring_slo_total_service_filter">
    <rdfs:label>total_service_filter</rdfs:label>
    <rdfs:comment>A TimeSeries [monitoring filter](https://cloud.google.com/monitoring/api/v3/filters)
quantifying total demanded service.

Must have ValueType = DOUBLE or ValueType = INT64 and
must have MetricKind = DELTA or MetricKind = CUMULATIVE.

Exactly two of 'good_service_filter','bad_service_filter','total_service_filter'
must be set (good + bad = total is assumed).</rdfs:comment>
    <rdfs:domain rdf:resource="http://example.org/onto/class/google_monitoring_slo"/>
    <rdfs:range rdf:resource="http://www.w3.org/2001/XMLSchema#string"/>
  </owl:DatatypeProperty>
  <owl:DatatypeProperty rdf:about="http://example.org/onto/prop/google_monitoring_slo_create">
    <rdfs:label>create</rdfs:label>
    <rdfs:domain rdf:resource="http://example.org/onto/class/google_monitoring_slo"/>
    <rdfs:range rdf:resource="http://www.w3.org/2001/XMLSchema#string"/>
  </owl:DatatypeProperty>
  <owl:DatatypeProperty rdf:about="http://example.org/onto/prop/google_monitoring_slo_delete">
    <rdfs:label>delete</rdfs:label>
    <rdfs:domain rdf:resource="http://example.org/onto/class/google_monitoring_slo"/>
    <rdfs:range rdf:resource="http://www.w3.org/2001/XMLSchema#string"/>
  </owl:DatatypeProperty>
  <owl:DatatypeProperty rdf:about="http://example.org/onto/prop/google_monitoring_slo_update">
    <rdfs:label>update</rdfs:label>
    <rdfs:domain rdf:resource="http://example.org/onto/class/google_monitoring_slo"/>
    <rdfs:range rdf:resource="http://www.w3.org/2001/XMLSchema#string"/>
  </owl:DatatypeProperty>
  <owl:DatatypeProperty rdf:about="http://example.org/onto/prop/google_monitoring_slo_good_bad_metric_filter">
    <rdfs:label>good_bad_metric_filter</rdfs:label>
    <rdfs:comment>A TimeSeries [monitoring filter](https://cloud.google.com/monitoring/api/v3/filters)
with ValueType = BOOL. The window is good if any true values
appear in the window. One of 'good_bad_metric_filter',
'good_total_ratio_threshold', 'metric_mean_in_range',
'metric_sum_in_range' must be set for 'windows_based_sli'.</rdfs:comment>
    <rdfs:domain rdf:resource="http://example.org/onto/class/google_monitoring_slo"/>
    <rdfs:range rdf:resource="http://www.w3.org/2001/XMLSchema#string"/>
  </owl:DatatypeProperty>
  <owl:DatatypeProperty rdf:about="http://example.org/onto/prop/google_monitoring_slo_window_period">
    <rdfs:label>window_period</rdfs:label>
    <rdfs:comment>Duration over which window quality is evaluated, given as a
duration string "{X}s" representing X seconds. Must be an
integer fraction of a day and at least 60s.</rdfs:comment>
    <rdfs:domain rdf:resource="http://example.org/onto/class/google_monitoring_slo"/>
    <rdfs:range rdf:resource="http://www.w3.org/2001/XMLSchema#string"/>
  </owl:DatatypeProperty>
  <owl:DatatypeProperty rdf:about="http://example.org/onto/prop/google_monitoring_slo_threshold">
    <rdfs:label>threshold</rdfs:label>
    <rdfs:comment>If window performance >= threshold, the window is counted
as good.</rdfs:comment>
    <rdfs:domain rdf:resource="http://example.org/onto/class/google_monitoring_slo"/>
    <rdfs:range rdf:resource="http://www.w3.org/2001/XMLSchema#string"/>
  </owl:DatatypeProperty>
  <owl:DatatypeProperty rdf:about="http://example.org/onto/prop/google_monitoring_slo_location">
    <rdfs:label>location</rdfs:label>
    <rdfs:comment>An optional set of locations to which this SLI is relevant.
Telemetry from other locations will not be used to calculate
performance for this SLI. If omitted, this SLI applies to all
locations in which the Service has activity. For service types
that don't support breaking down by location, setting this
field will result in an error.</rdfs:comment>
    <rdfs:domain rdf:resource="http://example.org/onto/class/google_monitoring_slo"/>
    <rdfs:range rdf:resource="http://www.w3.org/2001/XMLSchema#string"/>
  </owl:DatatypeProperty>
  <owl:DatatypeProperty rdf:about="http://example.org/onto/prop/google_monitoring_slo_method">
    <rdfs:label>method</rdfs:label>
    <rdfs:comment>An optional set of RPCs to which this SLI is relevant.
Telemetry from other methods will not be used to calculate
performance for this SLI. If omitted, this SLI applies to all
the Service's methods. For service types that don't support
breaking down by method, setting this field will result in an
error.</rdfs:comment>
    <rdfs:domain rdf:resource="http://example.org/onto/class/google_monitoring_slo"/>
    <rdfs:range rdf:resource="http://www.w3.org/2001/XMLSchema#string"/>
  </owl:DatatypeProperty>
  <owl:DatatypeProperty rdf:about="http://example.org/onto/prop/google_monitoring_slo_version">
    <rdfs:label>version</rdfs:label>
    <rdfs:comment>The set of API versions to which this SLI is relevant.
Telemetry from other API versions will not be used to
calculate performance for this SLI. If omitted,
this SLI applies to all API versions. For service types
that don't support breaking down by version, setting this
field will result in an error.</rdfs:comment>
    <rdfs:domain rdf:resource="http://example.org/onto/class/google_monitoring_slo"/>
    <rdfs:range rdf:resource="http://www.w3.org/2001/XMLSchema#string"/>
  </owl:DatatypeProperty>
  <owl:DatatypeProperty rdf:about="http://example.org/onto/prop/google_monitoring_slo_enabled">
    <rdfs:label>enabled</rdfs:label>
    <rdfs:comment>Whether an availability SLI is enabled or not. Must be set to 'true. Defaults to 'true'.</rdfs:comment>
    <rdfs:domain rdf:resource="http://example.org/onto/class/google_monitoring_slo"/>
    <rdfs:range rdf:resource="http://www.w3.org/2001/XMLSchema#string"/>
  </owl:DatatypeProperty>
  <owl:DatatypeProperty rdf:about="http://example.org/onto/prop/google_monitoring_slo_threshold">
    <rdfs:label>threshold</rdfs:label>
    <rdfs:comment>A duration string, e.g. 10s.
Good service is defined to be the count of requests made to
this service that return in no more than threshold.</rdfs:comment>
    <rdfs:domain rdf:resource="http://example.org/onto/class/google_monitoring_slo"/>
    <rdfs:range rdf:resource="http://www.w3.org/2001/XMLSchema#string"/>
  </owl:DatatypeProperty>
  <owl:DatatypeProperty rdf:about="http://example.org/onto/prop/google_monitoring_slo_distribution_filter">
    <rdfs:label>distribution_filter</rdfs:label>
    <rdfs:comment>A TimeSeries [monitoring filter](https://cloud.google.com/monitoring/api/v3/filters)
aggregating values to quantify the good service provided.

Must have ValueType = DISTRIBUTION and
MetricKind = DELTA or MetricKind = CUMULATIVE.</rdfs:comment>
    <rdfs:domain rdf:resource="http://example.org/onto/class/google_monitoring_slo"/>
    <rdfs:range rdf:resource="http://www.w3.org/2001/XMLSchema#string"/>
  </owl:DatatypeProperty>
  <owl:DatatypeProperty rdf:about="http://example.org/onto/prop/google_monitoring_slo_max">
    <rdfs:label>max</rdfs:label>
    <rdfs:comment>max value for the range (inclusive). If not given,
will be set to 0</rdfs:comment>
    <rdfs:domain rdf:resource="http://example.org/onto/class/google_monitoring_slo"/>
    <rdfs:range rdf:resource="http://www.w3.org/2001/XMLSchema#string"/>
  </owl:DatatypeProperty>
  <owl:DatatypeProperty rdf:about="http://example.org/onto/prop/google_monitoring_slo_min">
    <rdfs:label>min</rdfs:label>
    <rdfs:comment>Min value for the range (inclusive). If not given,
will be set to 0</rdfs:comment>
    <rdfs:domain rdf:resource="http://example.org/onto/class/google_monitoring_slo"/>
    <rdfs:range rdf:resource="http://www.w3.org/2001/XMLSchema#string"/>
  </owl:DatatypeProperty>
  <owl:DatatypeProperty rdf:about="http://example.org/onto/prop/google_monitoring_slo_bad_service_filter">
    <rdfs:label>bad_service_filter</rdfs:label>
    <rdfs:comment>A TimeSeries [monitoring filter](https://cloud.google.com/monitoring/api/v3/filters)
quantifying bad service provided, either demanded service that
was not provided or demanded service that was of inadequate
quality. Exactly two of
good, bad, or total service filter must be defined (where
good + bad = total is assumed)

Must have ValueType = DOUBLE or ValueType = INT64 and
must have MetricKind = DELTA or MetricKind = CUMULATIVE.</rdfs:comment>
    <rdfs:domain rdf:resource="http://example.org/onto/class/google_monitoring_slo"/>
    <rdfs:range rdf:resource="http://www.w3.org/2001/XMLSchema#string"/>
  </owl:DatatypeProperty>
  <owl:DatatypeProperty rdf:about="http://example.org/onto/prop/google_monitoring_slo_good_service_filter">
    <rdfs:label>good_service_filter</rdfs:label>
    <rdfs:comment>A TimeSeries [monitoring filter](https://cloud.google.com/monitoring/api/v3/filters)
quantifying good service provided. Exactly two of
good, bad, or total service filter must be defined (where
good + bad = total is assumed)

Must have ValueType = DOUBLE or ValueType = INT64 and
must have MetricKind = DELTA or MetricKind = CUMULATIVE.</rdfs:comment>
    <rdfs:domain rdf:resource="http://example.org/onto/class/google_monitoring_slo"/>
    <rdfs:range rdf:resource="http://www.w3.org/2001/XMLSchema#string"/>
  </owl:DatatypeProperty>
  <owl:DatatypeProperty rdf:about="http://example.org/onto/prop/google_monitoring_slo_total_service_filter">
    <rdfs:label>total_service_filter</rdfs:label>
    <rdfs:comment>A TimeSeries [monitoring filter](https://cloud.google.com/monitoring/api/v3/filters)
quantifying total demanded service. Exactly two of
good, bad, or total service filter must be defined (where
good + bad = total is assumed)

Must have ValueType = DOUBLE or ValueType = INT64 and
must have MetricKind = DELTA or MetricKind = CUMULATIVE.</rdfs:comment>
    <rdfs:domain rdf:resource="http://example.org/onto/class/google_monitoring_slo"/>
    <rdfs:range rdf:resource="http://www.w3.org/2001/XMLSchema#string"/>
  </owl:DatatypeProperty>
  <owl:DatatypeProperty rdf:about="http://example.org/onto/prop/google_monitoring_slo_time_series">
    <rdfs:label>time_series</rdfs:label>
    <rdfs:comment>A [monitoring filter](https://cloud.google.com/monitoring/api/v3/filters)
specifying the TimeSeries to use for evaluating window
The provided TimeSeries must have ValueType = INT64 or
ValueType = DOUBLE and MetricKind = GAUGE. Mean value 'X'
should satisfy 'range.min <= X <= range.max'
under good service.</rdfs:comment>
    <rdfs:domain rdf:resource="http://example.org/onto/class/google_monitoring_slo"/>
    <rdfs:range rdf:resource="http://www.w3.org/2001/XMLSchema#string"/>
  </owl:DatatypeProperty>
  <owl:DatatypeProperty rdf:about="http://example.org/onto/prop/google_monitoring_slo_max">
    <rdfs:label>max</rdfs:label>
    <rdfs:comment>max value for the range (inclusive). If not given,
will be set to "infinity", defining an open range
">= range.min"</rdfs:comment>
    <rdfs:domain rdf:resource="http://example.org/onto/class/google_monitoring_slo"/>
    <rdfs:range rdf:resource="http://www.w3.org/2001/XMLSchema#string"/>
  </owl:DatatypeProperty>
  <owl:DatatypeProperty rdf:about="http://example.org/onto/prop/google_monitoring_slo_min">
    <rdfs:label>min</rdfs:label>
    <rdfs:comment>Min value for the range (inclusive). If not given,
will be set to "-infinity", defining an open range
"< range.max"</rdfs:comment>
    <rdfs:domain rdf:resource="http://example.org/onto/class/google_monitoring_slo"/>
    <rdfs:range rdf:resource="http://www.w3.org/2001/XMLSchema#string"/>
  </owl:DatatypeProperty>
  <owl:DatatypeProperty rdf:about="http://example.org/onto/prop/google_monitoring_slo_time_series">
    <rdfs:label>time_series</rdfs:label>
    <rdfs:comment>A [monitoring filter](https://cloud.google.com/monitoring/api/v3/filters)
specifying the TimeSeries to use for evaluating window
quality. The provided TimeSeries must have
ValueType = INT64 or ValueType = DOUBLE and
MetricKind = GAUGE.

Summed value 'X' should satisfy
'range.min <= X <= range.max' for a good window.</rdfs:comment>
    <rdfs:domain rdf:resource="http://example.org/onto/class/google_monitoring_slo"/>
    <rdfs:range rdf:resource="http://www.w3.org/2001/XMLSchema#string"/>
  </owl:DatatypeProperty>
  <owl:DatatypeProperty rdf:about="http://example.org/onto/prop/google_monitoring_slo_max">
    <rdfs:label>max</rdfs:label>
    <rdfs:comment>max value for the range (inclusive). If not given,
will be set to "infinity", defining an open range
">= range.min"</rdfs:comment>
    <rdfs:domain rdf:resource="http://example.org/onto/class/google_monitoring_slo"/>
    <rdfs:range rdf:resource="http://www.w3.org/2001/XMLSchema#string"/>
  </owl:DatatypeProperty>
  <owl:DatatypeProperty rdf:about="http://example.org/onto/prop/google_monitoring_slo_min">
    <rdfs:label>min</rdfs:label>
    <rdfs:comment>Min value for the range (inclusive). If not given,
will be set to "-infinity", defining an open range
"< range.max"</rdfs:comment>
    <rdfs:domain rdf:resource="http://example.org/onto/class/google_monitoring_slo"/>
    <rdfs:range rdf:resource="http://www.w3.org/2001/XMLSchema#string"/>
  </owl:DatatypeProperty>
</rdf:RDF>
