<?xml version="1.0" encoding="UTF-8"?>
<rdf:RDF
  xmlns:rdf="http://www.w3.org/1999/02/22-rdf-syntax-ns#"
  xmlns:rdfs="http://www.w3.org/2000/01/rdf-schema#"
  xmlns:owl="http://www.w3.org/2002/07/owl#"
  xmlns:xsd="http://www.w3.org/2001/XMLSchema#"
  xml:base="http://example.org/onto/">
  <owl:Class rdf:about="http://example.org/onto/class/google_dataproc_job">
    <rdfs:label>google_dataproc_job</rdfs:label>
    <rdfs:comment>#
#     ***     AUTO GENERATED CODE    ***    Type: Handwritten     ***
#
# ----------------------------------------------------------------------------
#
#     This code is generated by Magic Modules using the following:
#
#     Source file: https://github.com/GoogleCloudPlatform/magic-modules/tree/main/mmv1/third_party/terraform/website/docs/r/dataproc_job.html.markdown
#
#     DO NOT EDIT this file directly. Any changes made to this file will be
#     overwritten during the next generation cycle.
#
# ----------------------------------------------------------------------------
subcategory: "Dataproc"
description: |-
  Manages a job resource within a Dataproc cluster.
---</rdfs:comment>
  </owl:Class>
  <owl:DatatypeProperty rdf:about="http://example.org/onto/prop/google_dataproc_job_driver_controls_files_uri">
    <rdfs:label>driver_controls_files_uri</rdfs:label>
    <rdfs:comment>Output-only. If present, the location of miscellaneous control files which may be used as part of job setup and handling. If not present, control files may be placed in the same location as driver_output_uri.</rdfs:comment>
    <rdfs:domain rdf:resource="http://example.org/onto/class/google_dataproc_job"/>
    <rdfs:range rdf:resource="http://www.w3.org/2001/XMLSchema#string"/>
  </owl:DatatypeProperty>
  <owl:DatatypeProperty rdf:about="http://example.org/onto/prop/google_dataproc_job_driver_output_resource_uri">
    <rdfs:label>driver_output_resource_uri</rdfs:label>
    <rdfs:comment>Output-only. A URI pointing to the location of the stdout of the job's driver program</rdfs:comment>
    <rdfs:domain rdf:resource="http://example.org/onto/class/google_dataproc_job"/>
    <rdfs:range rdf:resource="http://www.w3.org/2001/XMLSchema#string"/>
  </owl:DatatypeProperty>
  <owl:DatatypeProperty rdf:about="http://example.org/onto/prop/google_dataproc_job_effective_labels">
    <rdfs:label>effective_labels</rdfs:label>
    <rdfs:comment>All of labels (key/value pairs) present on the resource in GCP, including the labels configured through Terraform, other clients and services.</rdfs:comment>
    <rdfs:domain rdf:resource="http://example.org/onto/class/google_dataproc_job"/>
    <rdfs:range rdf:resource="http://www.w3.org/2001/XMLSchema#string"/>
  </owl:DatatypeProperty>
  <owl:DatatypeProperty rdf:about="http://example.org/onto/prop/google_dataproc_job_force_delete">
    <rdfs:label>force_delete</rdfs:label>
    <rdfs:comment>By default, you can only delete inactive jobs within Dataproc. Setting this to true, and calling destroy, will ensure that the job is first cancelled before issuing the delete.</rdfs:comment>
    <rdfs:domain rdf:resource="http://example.org/onto/class/google_dataproc_job"/>
    <rdfs:range rdf:resource="http://www.w3.org/2001/XMLSchema#string"/>
  </owl:DatatypeProperty>
  <owl:DatatypeProperty rdf:about="http://example.org/onto/prop/google_dataproc_job_id">
    <rdfs:label>id</rdfs:label>
    <rdfs:domain rdf:resource="http://example.org/onto/class/google_dataproc_job"/>
    <rdfs:range rdf:resource="http://www.w3.org/2001/XMLSchema#string"/>
  </owl:DatatypeProperty>
  <owl:DatatypeProperty rdf:about="http://example.org/onto/prop/google_dataproc_job_labels">
    <rdfs:label>labels</rdfs:label>
    <rdfs:comment>Optional. The labels to associate with this job.

				**Note**: This field is non-authoritative, and will only manage the labels present in your configuration.
				Please refer to the field 'effective_labels' for all of the labels present on the resource.</rdfs:comment>
    <rdfs:domain rdf:resource="http://example.org/onto/class/google_dataproc_job"/>
    <rdfs:range rdf:resource="http://www.w3.org/2001/XMLSchema#string"/>
  </owl:DatatypeProperty>
  <owl:DatatypeProperty rdf:about="http://example.org/onto/prop/google_dataproc_job_project">
    <rdfs:label>project</rdfs:label>
    <rdfs:comment>The project in which the cluster can be found and jobs subsequently run against. If it is not provided, the provider project is used.</rdfs:comment>
    <rdfs:domain rdf:resource="http://example.org/onto/class/google_dataproc_job"/>
    <rdfs:range rdf:resource="http://www.w3.org/2001/XMLSchema#string"/>
  </owl:DatatypeProperty>
  <owl:DatatypeProperty rdf:about="http://example.org/onto/prop/google_dataproc_job_region">
    <rdfs:label>region</rdfs:label>
    <rdfs:comment>The Cloud Dataproc region. This essentially determines which clusters are available for this job to be submitted to. If not specified, defaults to global.</rdfs:comment>
    <rdfs:domain rdf:resource="http://example.org/onto/class/google_dataproc_job"/>
    <rdfs:range rdf:resource="http://www.w3.org/2001/XMLSchema#string"/>
  </owl:DatatypeProperty>
  <owl:DatatypeProperty rdf:about="http://example.org/onto/prop/google_dataproc_job_status">
    <rdfs:label>status</rdfs:label>
    <rdfs:comment>The status of the job.</rdfs:comment>
    <rdfs:domain rdf:resource="http://example.org/onto/class/google_dataproc_job"/>
    <rdfs:range rdf:resource="http://www.w3.org/2001/XMLSchema#string"/>
  </owl:DatatypeProperty>
  <owl:DatatypeProperty rdf:about="http://example.org/onto/prop/google_dataproc_job_terraform_labels">
    <rdfs:label>terraform_labels</rdfs:label>
    <rdfs:comment>The combination of labels configured directly on the resource and default labels configured on the provider.</rdfs:comment>
    <rdfs:domain rdf:resource="http://example.org/onto/class/google_dataproc_job"/>
    <rdfs:range rdf:resource="http://www.w3.org/2001/XMLSchema#string"/>
  </owl:DatatypeProperty>
  <owl:DatatypeProperty rdf:about="http://example.org/onto/prop/google_dataproc_job_archive_uris">
    <rdfs:label>archive_uris</rdfs:label>
    <rdfs:comment>HCFS URIs of archives to be extracted in the working directory of .jar, .tar, .tar.gz, .tgz, and .zip.</rdfs:comment>
    <rdfs:domain rdf:resource="http://example.org/onto/class/google_dataproc_job"/>
    <rdfs:range rdf:resource="http://www.w3.org/2001/XMLSchema#string"/>
  </owl:DatatypeProperty>
  <owl:DatatypeProperty rdf:about="http://example.org/onto/prop/google_dataproc_job_args">
    <rdfs:label>args</rdfs:label>
    <rdfs:comment>The arguments to pass to the driver.</rdfs:comment>
    <rdfs:domain rdf:resource="http://example.org/onto/class/google_dataproc_job"/>
    <rdfs:range rdf:resource="http://www.w3.org/2001/XMLSchema#string"/>
  </owl:DatatypeProperty>
  <owl:DatatypeProperty rdf:about="http://example.org/onto/prop/google_dataproc_job_file_uris">
    <rdfs:label>file_uris</rdfs:label>
    <rdfs:comment>HCFS URIs of files to be copied to the working directory of Spark drivers and distributed tasks. Useful for naively parallel tasks.</rdfs:comment>
    <rdfs:domain rdf:resource="http://example.org/onto/class/google_dataproc_job"/>
    <rdfs:range rdf:resource="http://www.w3.org/2001/XMLSchema#string"/>
  </owl:DatatypeProperty>
  <owl:DatatypeProperty rdf:about="http://example.org/onto/prop/google_dataproc_job_jar_file_uris">
    <rdfs:label>jar_file_uris</rdfs:label>
    <rdfs:comment>HCFS URIs of jar files to add to the CLASSPATHs of the Spark driver and tasks.</rdfs:comment>
    <rdfs:domain rdf:resource="http://example.org/onto/class/google_dataproc_job"/>
    <rdfs:range rdf:resource="http://www.w3.org/2001/XMLSchema#string"/>
  </owl:DatatypeProperty>
  <owl:DatatypeProperty rdf:about="http://example.org/onto/prop/google_dataproc_job_main_class">
    <rdfs:label>main_class</rdfs:label>
    <rdfs:comment>The class containing the main method of the driver. Must be in a provided jar or jar that is already on the classpath. Conflicts with main_jar_file_uri</rdfs:comment>
    <rdfs:domain rdf:resource="http://example.org/onto/class/google_dataproc_job"/>
    <rdfs:range rdf:resource="http://www.w3.org/2001/XMLSchema#string"/>
  </owl:DatatypeProperty>
  <owl:DatatypeProperty rdf:about="http://example.org/onto/prop/google_dataproc_job_main_jar_file_uri">
    <rdfs:label>main_jar_file_uri</rdfs:label>
    <rdfs:comment>The HCFS URI of jar file containing the driver jar. Conflicts with main_class</rdfs:comment>
    <rdfs:domain rdf:resource="http://example.org/onto/class/google_dataproc_job"/>
    <rdfs:range rdf:resource="http://www.w3.org/2001/XMLSchema#string"/>
  </owl:DatatypeProperty>
  <owl:DatatypeProperty rdf:about="http://example.org/onto/prop/google_dataproc_job_properties">
    <rdfs:label>properties</rdfs:label>
    <rdfs:comment>A mapping of property names to values, used to configure Spark. Properties that conflict with values set by the Cloud Dataproc API may be overwritten. Can include properties set in /etc/spark/conf/spark-defaults.conf and classes in user code.</rdfs:comment>
    <rdfs:domain rdf:resource="http://example.org/onto/class/google_dataproc_job"/>
    <rdfs:range rdf:resource="http://www.w3.org/2001/XMLSchema#string"/>
  </owl:DatatypeProperty>
  <owl:DatatypeProperty rdf:about="http://example.org/onto/prop/google_dataproc_job_driver_log_levels">
    <rdfs:label>driver_log_levels</rdfs:label>
    <rdfs:comment>Optional. The per-package log levels for the driver. This may include 'root' package name to configure rootLogger. Examples: 'com.google = FATAL', 'root = INFO', 'org.apache = DEBUG'.</rdfs:comment>
    <rdfs:domain rdf:resource="http://example.org/onto/class/google_dataproc_job"/>
    <rdfs:range rdf:resource="http://www.w3.org/2001/XMLSchema#string"/>
  </owl:DatatypeProperty>
  <owl:DatatypeProperty rdf:about="http://example.org/onto/prop/google_dataproc_job_continue_on_failure">
    <rdfs:label>continue_on_failure</rdfs:label>
    <rdfs:comment>Whether to continue executing queries if a query fails. The default value is false. Setting to true can be useful when executing independent parallel queries. Defaults to false.</rdfs:comment>
    <rdfs:domain rdf:resource="http://example.org/onto/class/google_dataproc_job"/>
    <rdfs:range rdf:resource="http://www.w3.org/2001/XMLSchema#string"/>
  </owl:DatatypeProperty>
  <owl:DatatypeProperty rdf:about="http://example.org/onto/prop/google_dataproc_job_jar_file_uris">
    <rdfs:label>jar_file_uris</rdfs:label>
    <rdfs:comment>HCFS URIs of jar files to add to the CLASSPATH of the Hive server and Hadoop MapReduce (MR) tasks. Can contain Hive SerDes and UDFs.</rdfs:comment>
    <rdfs:domain rdf:resource="http://example.org/onto/class/google_dataproc_job"/>
    <rdfs:range rdf:resource="http://www.w3.org/2001/XMLSchema#string"/>
  </owl:DatatypeProperty>
  <owl:DatatypeProperty rdf:about="http://example.org/onto/prop/google_dataproc_job_properties">
    <rdfs:label>properties</rdfs:label>
    <rdfs:comment>A mapping of property names and values, used to configure Hive. Properties that conflict with values set by the Cloud Dataproc API may be overwritten. Can include properties set in /etc/hadoop/conf/*-site.xml, /etc/hive/conf/hive-site.xml, and classes in user code.</rdfs:comment>
    <rdfs:domain rdf:resource="http://example.org/onto/class/google_dataproc_job"/>
    <rdfs:range rdf:resource="http://www.w3.org/2001/XMLSchema#string"/>
  </owl:DatatypeProperty>
  <owl:DatatypeProperty rdf:about="http://example.org/onto/prop/google_dataproc_job_query_file_uri">
    <rdfs:label>query_file_uri</rdfs:label>
    <rdfs:comment>HCFS URI of file containing Hive script to execute as the job. Conflicts with query_list</rdfs:comment>
    <rdfs:domain rdf:resource="http://example.org/onto/class/google_dataproc_job"/>
    <rdfs:range rdf:resource="http://www.w3.org/2001/XMLSchema#string"/>
  </owl:DatatypeProperty>
  <owl:DatatypeProperty rdf:about="http://example.org/onto/prop/google_dataproc_job_query_list">
    <rdfs:label>query_list</rdfs:label>
    <rdfs:comment>The list of Hive queries or statements to execute as part of the job. Conflicts with query_file_uri</rdfs:comment>
    <rdfs:domain rdf:resource="http://example.org/onto/class/google_dataproc_job"/>
    <rdfs:range rdf:resource="http://www.w3.org/2001/XMLSchema#string"/>
  </owl:DatatypeProperty>
  <owl:DatatypeProperty rdf:about="http://example.org/onto/prop/google_dataproc_job_script_variables">
    <rdfs:label>script_variables</rdfs:label>
    <rdfs:comment>Mapping of query variable names to values (equivalent to the Hive command: SET name="value";).</rdfs:comment>
    <rdfs:domain rdf:resource="http://example.org/onto/class/google_dataproc_job"/>
    <rdfs:range rdf:resource="http://www.w3.org/2001/XMLSchema#string"/>
  </owl:DatatypeProperty>
  <owl:DatatypeProperty rdf:about="http://example.org/onto/prop/google_dataproc_job_continue_on_failure">
    <rdfs:label>continue_on_failure</rdfs:label>
    <rdfs:comment>Whether to continue executing queries if a query fails. The default value is false. Setting to true can be useful when executing independent parallel queries. Defaults to false.</rdfs:comment>
    <rdfs:domain rdf:resource="http://example.org/onto/class/google_dataproc_job"/>
    <rdfs:range rdf:resource="http://www.w3.org/2001/XMLSchema#string"/>
  </owl:DatatypeProperty>
  <owl:DatatypeProperty rdf:about="http://example.org/onto/prop/google_dataproc_job_jar_file_uris">
    <rdfs:label>jar_file_uris</rdfs:label>
    <rdfs:comment>HCFS URIs of jar files to add to the CLASSPATH of the Pig Client and Hadoop MapReduce (MR) tasks. Can contain Pig UDFs.</rdfs:comment>
    <rdfs:domain rdf:resource="http://example.org/onto/class/google_dataproc_job"/>
    <rdfs:range rdf:resource="http://www.w3.org/2001/XMLSchema#string"/>
  </owl:DatatypeProperty>
  <owl:DatatypeProperty rdf:about="http://example.org/onto/prop/google_dataproc_job_properties">
    <rdfs:label>properties</rdfs:label>
    <rdfs:comment>A mapping of property names to values, used to configure Pig. Properties that conflict with values set by the Cloud Dataproc API may be overwritten. Can include properties set in /etc/hadoop/conf/*-site.xml, /etc/pig/conf/pig.properties, and classes in user code.</rdfs:comment>
    <rdfs:domain rdf:resource="http://example.org/onto/class/google_dataproc_job"/>
    <rdfs:range rdf:resource="http://www.w3.org/2001/XMLSchema#string"/>
  </owl:DatatypeProperty>
  <owl:DatatypeProperty rdf:about="http://example.org/onto/prop/google_dataproc_job_query_file_uri">
    <rdfs:label>query_file_uri</rdfs:label>
    <rdfs:comment>HCFS URI of file containing Hive script to execute as the job. Conflicts with query_list</rdfs:comment>
    <rdfs:domain rdf:resource="http://example.org/onto/class/google_dataproc_job"/>
    <rdfs:range rdf:resource="http://www.w3.org/2001/XMLSchema#string"/>
  </owl:DatatypeProperty>
  <owl:DatatypeProperty rdf:about="http://example.org/onto/prop/google_dataproc_job_query_list">
    <rdfs:label>query_list</rdfs:label>
    <rdfs:comment>The list of Hive queries or statements to execute as part of the job. Conflicts with query_file_uri</rdfs:comment>
    <rdfs:domain rdf:resource="http://example.org/onto/class/google_dataproc_job"/>
    <rdfs:range rdf:resource="http://www.w3.org/2001/XMLSchema#string"/>
  </owl:DatatypeProperty>
  <owl:DatatypeProperty rdf:about="http://example.org/onto/prop/google_dataproc_job_script_variables">
    <rdfs:label>script_variables</rdfs:label>
    <rdfs:comment>Mapping of query variable names to values (equivalent to the Pig command: name=[value]).</rdfs:comment>
    <rdfs:domain rdf:resource="http://example.org/onto/class/google_dataproc_job"/>
    <rdfs:range rdf:resource="http://www.w3.org/2001/XMLSchema#string"/>
  </owl:DatatypeProperty>
  <owl:DatatypeProperty rdf:about="http://example.org/onto/prop/google_dataproc_job_driver_log_levels">
    <rdfs:label>driver_log_levels</rdfs:label>
    <rdfs:comment>Optional. The per-package log levels for the driver. This may include 'root' package name to configure rootLogger. Examples: 'com.google = FATAL', 'root = INFO', 'org.apache = DEBUG'.</rdfs:comment>
    <rdfs:domain rdf:resource="http://example.org/onto/class/google_dataproc_job"/>
    <rdfs:range rdf:resource="http://www.w3.org/2001/XMLSchema#string"/>
  </owl:DatatypeProperty>
  <owl:DatatypeProperty rdf:about="http://example.org/onto/prop/google_dataproc_job_cluster_name">
    <rdfs:label>cluster_name</rdfs:label>
    <rdfs:comment>The name of the cluster where the job will be submitted</rdfs:comment>
    <rdfs:domain rdf:resource="http://example.org/onto/class/google_dataproc_job"/>
    <rdfs:range rdf:resource="http://www.w3.org/2001/XMLSchema#string"/>
  </owl:DatatypeProperty>
  <owl:DatatypeProperty rdf:about="http://example.org/onto/prop/google_dataproc_job_cluster_uuid">
    <rdfs:label>cluster_uuid</rdfs:label>
    <rdfs:comment>Output-only. A cluster UUID generated by the Cloud Dataproc service when the job is submitted</rdfs:comment>
    <rdfs:domain rdf:resource="http://example.org/onto/class/google_dataproc_job"/>
    <rdfs:range rdf:resource="http://www.w3.org/2001/XMLSchema#string"/>
  </owl:DatatypeProperty>
  <owl:DatatypeProperty rdf:about="http://example.org/onto/prop/google_dataproc_job_client_tags">
    <rdfs:label>client_tags</rdfs:label>
    <rdfs:comment>Presto client tags to attach to this query.</rdfs:comment>
    <rdfs:domain rdf:resource="http://example.org/onto/class/google_dataproc_job"/>
    <rdfs:range rdf:resource="http://www.w3.org/2001/XMLSchema#string"/>
  </owl:DatatypeProperty>
  <owl:DatatypeProperty rdf:about="http://example.org/onto/prop/google_dataproc_job_continue_on_failure">
    <rdfs:label>continue_on_failure</rdfs:label>
    <rdfs:comment>Whether to continue executing queries if a query fails. Setting to true can be useful when executing independent parallel queries. Defaults to false.</rdfs:comment>
    <rdfs:domain rdf:resource="http://example.org/onto/class/google_dataproc_job"/>
    <rdfs:range rdf:resource="http://www.w3.org/2001/XMLSchema#string"/>
  </owl:DatatypeProperty>
  <owl:DatatypeProperty rdf:about="http://example.org/onto/prop/google_dataproc_job_output_format">
    <rdfs:label>output_format</rdfs:label>
    <rdfs:comment>The format in which query output will be displayed. See the Presto documentation for supported output formats.</rdfs:comment>
    <rdfs:domain rdf:resource="http://example.org/onto/class/google_dataproc_job"/>
    <rdfs:range rdf:resource="http://www.w3.org/2001/XMLSchema#string"/>
  </owl:DatatypeProperty>
  <owl:DatatypeProperty rdf:about="http://example.org/onto/prop/google_dataproc_job_properties">
    <rdfs:label>properties</rdfs:label>
    <rdfs:comment>A mapping of property names to values. Used to set Presto session properties Equivalent to using the --session flag in the Presto CLI.</rdfs:comment>
    <rdfs:domain rdf:resource="http://example.org/onto/class/google_dataproc_job"/>
    <rdfs:range rdf:resource="http://www.w3.org/2001/XMLSchema#string"/>
  </owl:DatatypeProperty>
  <owl:DatatypeProperty rdf:about="http://example.org/onto/prop/google_dataproc_job_query_file_uri">
    <rdfs:label>query_file_uri</rdfs:label>
    <rdfs:comment>The HCFS URI of the script that contains SQL queries. Conflicts with query_list</rdfs:comment>
    <rdfs:domain rdf:resource="http://example.org/onto/class/google_dataproc_job"/>
    <rdfs:range rdf:resource="http://www.w3.org/2001/XMLSchema#string"/>
  </owl:DatatypeProperty>
  <owl:DatatypeProperty rdf:about="http://example.org/onto/prop/google_dataproc_job_query_list">
    <rdfs:label>query_list</rdfs:label>
    <rdfs:comment>The list of SQL queries or statements to execute as part of the job. Conflicts with query_file_uri</rdfs:comment>
    <rdfs:domain rdf:resource="http://example.org/onto/class/google_dataproc_job"/>
    <rdfs:range rdf:resource="http://www.w3.org/2001/XMLSchema#string"/>
  </owl:DatatypeProperty>
  <owl:DatatypeProperty rdf:about="http://example.org/onto/prop/google_dataproc_job_driver_log_levels">
    <rdfs:label>driver_log_levels</rdfs:label>
    <rdfs:comment>Optional. The per-package log levels for the driver. This may include 'root' package name to configure rootLogger. Examples: 'com.google = FATAL', 'root = INFO', 'org.apache = DEBUG'.</rdfs:comment>
    <rdfs:domain rdf:resource="http://example.org/onto/class/google_dataproc_job"/>
    <rdfs:range rdf:resource="http://www.w3.org/2001/XMLSchema#string"/>
  </owl:DatatypeProperty>
  <owl:DatatypeProperty rdf:about="http://example.org/onto/prop/google_dataproc_job_archive_uris">
    <rdfs:label>archive_uris</rdfs:label>
    <rdfs:comment>Optional. HCFS URIs of archives to be extracted in the working directory of .jar, .tar, .tar.gz, .tgz, and .zip</rdfs:comment>
    <rdfs:domain rdf:resource="http://example.org/onto/class/google_dataproc_job"/>
    <rdfs:range rdf:resource="http://www.w3.org/2001/XMLSchema#string"/>
  </owl:DatatypeProperty>
  <owl:DatatypeProperty rdf:about="http://example.org/onto/prop/google_dataproc_job_args">
    <rdfs:label>args</rdfs:label>
    <rdfs:comment>Optional. The arguments to pass to the driver. Do not include arguments, such as --conf, that can be set as job properties, since a collision may occur that causes an incorrect job submission</rdfs:comment>
    <rdfs:domain rdf:resource="http://example.org/onto/class/google_dataproc_job"/>
    <rdfs:range rdf:resource="http://www.w3.org/2001/XMLSchema#string"/>
  </owl:DatatypeProperty>
  <owl:DatatypeProperty rdf:about="http://example.org/onto/prop/google_dataproc_job_file_uris">
    <rdfs:label>file_uris</rdfs:label>
    <rdfs:comment>Optional. HCFS URIs of files to be copied to the working directory of Python drivers and distributed tasks. Useful for naively parallel tasks</rdfs:comment>
    <rdfs:domain rdf:resource="http://example.org/onto/class/google_dataproc_job"/>
    <rdfs:range rdf:resource="http://www.w3.org/2001/XMLSchema#string"/>
  </owl:DatatypeProperty>
  <owl:DatatypeProperty rdf:about="http://example.org/onto/prop/google_dataproc_job_jar_file_uris">
    <rdfs:label>jar_file_uris</rdfs:label>
    <rdfs:comment>Optional. HCFS URIs of jar files to add to the CLASSPATHs of the Python driver and tasks</rdfs:comment>
    <rdfs:domain rdf:resource="http://example.org/onto/class/google_dataproc_job"/>
    <rdfs:range rdf:resource="http://www.w3.org/2001/XMLSchema#string"/>
  </owl:DatatypeProperty>
  <owl:DatatypeProperty rdf:about="http://example.org/onto/prop/google_dataproc_job_main_python_file_uri">
    <rdfs:label>main_python_file_uri</rdfs:label>
    <rdfs:comment>Required. The HCFS URI of the main Python file to use as the driver. Must be a .py file</rdfs:comment>
    <rdfs:domain rdf:resource="http://example.org/onto/class/google_dataproc_job"/>
    <rdfs:range rdf:resource="http://www.w3.org/2001/XMLSchema#string"/>
  </owl:DatatypeProperty>
  <owl:DatatypeProperty rdf:about="http://example.org/onto/prop/google_dataproc_job_properties">
    <rdfs:label>properties</rdfs:label>
    <rdfs:comment>Optional. A mapping of property names to values, used to configure PySpark. Properties that conflict with values set by the Cloud Dataproc API may be overwritten. Can include properties set in /etc/spark/conf/spark-defaults.conf and classes in user code</rdfs:comment>
    <rdfs:domain rdf:resource="http://example.org/onto/class/google_dataproc_job"/>
    <rdfs:range rdf:resource="http://www.w3.org/2001/XMLSchema#string"/>
  </owl:DatatypeProperty>
  <owl:DatatypeProperty rdf:about="http://example.org/onto/prop/google_dataproc_job_python_file_uris">
    <rdfs:label>python_file_uris</rdfs:label>
    <rdfs:comment>Optional. HCFS file URIs of Python files to pass to the PySpark framework. Supported file types: .py, .egg, and .zip</rdfs:comment>
    <rdfs:domain rdf:resource="http://example.org/onto/class/google_dataproc_job"/>
    <rdfs:range rdf:resource="http://www.w3.org/2001/XMLSchema#string"/>
  </owl:DatatypeProperty>
  <owl:DatatypeProperty rdf:about="http://example.org/onto/prop/google_dataproc_job_driver_log_levels">
    <rdfs:label>driver_log_levels</rdfs:label>
    <rdfs:comment>Optional. The per-package log levels for the driver. This may include 'root' package name to configure rootLogger. Examples: 'com.google = FATAL', 'root = INFO', 'org.apache = DEBUG'.</rdfs:comment>
    <rdfs:domain rdf:resource="http://example.org/onto/class/google_dataproc_job"/>
    <rdfs:range rdf:resource="http://www.w3.org/2001/XMLSchema#string"/>
  </owl:DatatypeProperty>
  <owl:DatatypeProperty rdf:about="http://example.org/onto/prop/google_dataproc_job_job_id">
    <rdfs:label>job_id</rdfs:label>
    <rdfs:comment>The job ID, which must be unique within the project. The job ID is generated by the server upon job submission or provided by the user as a means to perform retries without creating duplicate jobs</rdfs:comment>
    <rdfs:domain rdf:resource="http://example.org/onto/class/google_dataproc_job"/>
    <rdfs:range rdf:resource="http://www.w3.org/2001/XMLSchema#string"/>
  </owl:DatatypeProperty>
  <owl:DatatypeProperty rdf:about="http://example.org/onto/prop/google_dataproc_job_max_failures_per_hour">
    <rdfs:label>max_failures_per_hour</rdfs:label>
    <rdfs:comment>Maximum number of times per hour a driver may be restarted as a result of driver exiting with non-zero code before job is reported failed.</rdfs:comment>
    <rdfs:domain rdf:resource="http://example.org/onto/class/google_dataproc_job"/>
    <rdfs:range rdf:resource="http://www.w3.org/2001/XMLSchema#string"/>
  </owl:DatatypeProperty>
  <owl:DatatypeProperty rdf:about="http://example.org/onto/prop/google_dataproc_job_max_failures_total">
    <rdfs:label>max_failures_total</rdfs:label>
    <rdfs:comment>Maximum number of times in total a driver may be restarted as a result of driver exiting with non-zero code before job is reported failed.</rdfs:comment>
    <rdfs:domain rdf:resource="http://example.org/onto/class/google_dataproc_job"/>
    <rdfs:range rdf:resource="http://www.w3.org/2001/XMLSchema#string"/>
  </owl:DatatypeProperty>
  <owl:DatatypeProperty rdf:about="http://example.org/onto/prop/google_dataproc_job_archive_uris">
    <rdfs:label>archive_uris</rdfs:label>
    <rdfs:comment>HCFS URIs of archives to be extracted in the working directory of .jar, .tar, .tar.gz, .tgz, and .zip.</rdfs:comment>
    <rdfs:domain rdf:resource="http://example.org/onto/class/google_dataproc_job"/>
    <rdfs:range rdf:resource="http://www.w3.org/2001/XMLSchema#string"/>
  </owl:DatatypeProperty>
  <owl:DatatypeProperty rdf:about="http://example.org/onto/prop/google_dataproc_job_args">
    <rdfs:label>args</rdfs:label>
    <rdfs:comment>The arguments to pass to the driver.</rdfs:comment>
    <rdfs:domain rdf:resource="http://example.org/onto/class/google_dataproc_job"/>
    <rdfs:range rdf:resource="http://www.w3.org/2001/XMLSchema#string"/>
  </owl:DatatypeProperty>
  <owl:DatatypeProperty rdf:about="http://example.org/onto/prop/google_dataproc_job_file_uris">
    <rdfs:label>file_uris</rdfs:label>
    <rdfs:comment>HCFS URIs of files to be copied to the working directory of Spark drivers and distributed tasks. Useful for naively parallel tasks.</rdfs:comment>
    <rdfs:domain rdf:resource="http://example.org/onto/class/google_dataproc_job"/>
    <rdfs:range rdf:resource="http://www.w3.org/2001/XMLSchema#string"/>
  </owl:DatatypeProperty>
  <owl:DatatypeProperty rdf:about="http://example.org/onto/prop/google_dataproc_job_jar_file_uris">
    <rdfs:label>jar_file_uris</rdfs:label>
    <rdfs:comment>HCFS URIs of jar files to add to the CLASSPATHs of the Spark driver and tasks.</rdfs:comment>
    <rdfs:domain rdf:resource="http://example.org/onto/class/google_dataproc_job"/>
    <rdfs:range rdf:resource="http://www.w3.org/2001/XMLSchema#string"/>
  </owl:DatatypeProperty>
  <owl:DatatypeProperty rdf:about="http://example.org/onto/prop/google_dataproc_job_main_class">
    <rdfs:label>main_class</rdfs:label>
    <rdfs:comment>The class containing the main method of the driver. Must be in a provided jar or jar that is already on the classpath. Conflicts with main_jar_file_uri</rdfs:comment>
    <rdfs:domain rdf:resource="http://example.org/onto/class/google_dataproc_job"/>
    <rdfs:range rdf:resource="http://www.w3.org/2001/XMLSchema#string"/>
  </owl:DatatypeProperty>
  <owl:DatatypeProperty rdf:about="http://example.org/onto/prop/google_dataproc_job_main_jar_file_uri">
    <rdfs:label>main_jar_file_uri</rdfs:label>
    <rdfs:comment>The HCFS URI of jar file containing the driver jar. Conflicts with main_class</rdfs:comment>
    <rdfs:domain rdf:resource="http://example.org/onto/class/google_dataproc_job"/>
    <rdfs:range rdf:resource="http://www.w3.org/2001/XMLSchema#string"/>
  </owl:DatatypeProperty>
  <owl:DatatypeProperty rdf:about="http://example.org/onto/prop/google_dataproc_job_properties">
    <rdfs:label>properties</rdfs:label>
    <rdfs:comment>A mapping of property names to values, used to configure Spark. Properties that conflict with values set by the Cloud Dataproc API may be overwritten. Can include properties set in /etc/spark/conf/spark-defaults.conf and classes in user code.</rdfs:comment>
    <rdfs:domain rdf:resource="http://example.org/onto/class/google_dataproc_job"/>
    <rdfs:range rdf:resource="http://www.w3.org/2001/XMLSchema#string"/>
  </owl:DatatypeProperty>
  <owl:DatatypeProperty rdf:about="http://example.org/onto/prop/google_dataproc_job_driver_log_levels">
    <rdfs:label>driver_log_levels</rdfs:label>
    <rdfs:comment>Optional. The per-package log levels for the driver. This may include 'root' package name to configure rootLogger. Examples: 'com.google = FATAL', 'root = INFO', 'org.apache = DEBUG'.</rdfs:comment>
    <rdfs:domain rdf:resource="http://example.org/onto/class/google_dataproc_job"/>
    <rdfs:range rdf:resource="http://www.w3.org/2001/XMLSchema#string"/>
  </owl:DatatypeProperty>
  <owl:DatatypeProperty rdf:about="http://example.org/onto/prop/google_dataproc_job_jar_file_uris">
    <rdfs:label>jar_file_uris</rdfs:label>
    <rdfs:comment>HCFS URIs of jar files to be added to the Spark CLASSPATH.</rdfs:comment>
    <rdfs:domain rdf:resource="http://example.org/onto/class/google_dataproc_job"/>
    <rdfs:range rdf:resource="http://www.w3.org/2001/XMLSchema#string"/>
  </owl:DatatypeProperty>
  <owl:DatatypeProperty rdf:about="http://example.org/onto/prop/google_dataproc_job_properties">
    <rdfs:label>properties</rdfs:label>
    <rdfs:comment>A mapping of property names to values, used to configure Spark SQL's SparkConf. Properties that conflict with values set by the Cloud Dataproc API may be overwritten.</rdfs:comment>
    <rdfs:domain rdf:resource="http://example.org/onto/class/google_dataproc_job"/>
    <rdfs:range rdf:resource="http://www.w3.org/2001/XMLSchema#string"/>
  </owl:DatatypeProperty>
  <owl:DatatypeProperty rdf:about="http://example.org/onto/prop/google_dataproc_job_query_file_uri">
    <rdfs:label>query_file_uri</rdfs:label>
    <rdfs:comment>The HCFS URI of the script that contains SQL queries. Conflicts with query_list</rdfs:comment>
    <rdfs:domain rdf:resource="http://example.org/onto/class/google_dataproc_job"/>
    <rdfs:range rdf:resource="http://www.w3.org/2001/XMLSchema#string"/>
  </owl:DatatypeProperty>
  <owl:DatatypeProperty rdf:about="http://example.org/onto/prop/google_dataproc_job_query_list">
    <rdfs:label>query_list</rdfs:label>
    <rdfs:comment>The list of SQL queries or statements to execute as part of the job. Conflicts with query_file_uri</rdfs:comment>
    <rdfs:domain rdf:resource="http://example.org/onto/class/google_dataproc_job"/>
    <rdfs:range rdf:resource="http://www.w3.org/2001/XMLSchema#string"/>
  </owl:DatatypeProperty>
  <owl:DatatypeProperty rdf:about="http://example.org/onto/prop/google_dataproc_job_script_variables">
    <rdfs:label>script_variables</rdfs:label>
    <rdfs:comment>Mapping of query variable names to values (equivalent to the Spark SQL command: SET name="value";).</rdfs:comment>
    <rdfs:domain rdf:resource="http://example.org/onto/class/google_dataproc_job"/>
    <rdfs:range rdf:resource="http://www.w3.org/2001/XMLSchema#string"/>
  </owl:DatatypeProperty>
  <owl:DatatypeProperty rdf:about="http://example.org/onto/prop/google_dataproc_job_driver_log_levels">
    <rdfs:label>driver_log_levels</rdfs:label>
    <rdfs:comment>Optional. The per-package log levels for the driver. This may include 'root' package name to configure rootLogger. Examples: 'com.google = FATAL', 'root = INFO', 'org.apache = DEBUG'.</rdfs:comment>
    <rdfs:domain rdf:resource="http://example.org/onto/class/google_dataproc_job"/>
    <rdfs:range rdf:resource="http://www.w3.org/2001/XMLSchema#string"/>
  </owl:DatatypeProperty>
  <owl:DatatypeProperty rdf:about="http://example.org/onto/prop/google_dataproc_job_create">
    <rdfs:label>create</rdfs:label>
    <rdfs:domain rdf:resource="http://example.org/onto/class/google_dataproc_job"/>
    <rdfs:range rdf:resource="http://www.w3.org/2001/XMLSchema#string"/>
  </owl:DatatypeProperty>
  <owl:DatatypeProperty rdf:about="http://example.org/onto/prop/google_dataproc_job_delete">
    <rdfs:label>delete</rdfs:label>
    <rdfs:domain rdf:resource="http://example.org/onto/class/google_dataproc_job"/>
    <rdfs:range rdf:resource="http://www.w3.org/2001/XMLSchema#string"/>
  </owl:DatatypeProperty>
</rdf:RDF>
