<?xml version="1.0" encoding="UTF-8"?>
<rdf:RDF
  xmlns:rdf="http://www.w3.org/1999/02/22-rdf-syntax-ns#"
  xmlns:rdfs="http://www.w3.org/2000/01/rdf-schema#"
  xmlns:owl="http://www.w3.org/2002/07/owl#"
  xmlns:xsd="http://www.w3.org/2001/XMLSchema#"
  xml:base="http://example.org/onto/">
  <owl:Class rdf:about="http://example.org/onto/class/google_service_networking_connection">
    <rdfs:label>google_service_networking_connection</rdfs:label>
    <rdfs:comment>#
#     ***     AUTO GENERATED CODE    ***    Type: Handwritten     ***
#
# ----------------------------------------------------------------------------
#
#     This code is generated by Magic Modules using the following:
#
#     Source file: https://github.com/GoogleCloudPlatform/magic-modules/tree/main/mmv1/third_party/terraform/website/docs/r/service_networking_connection.html.markdown
#
#     DO NOT EDIT this file directly. Any changes made to this file will be
#     overwritten during the next generation cycle.
#
# ----------------------------------------------------------------------------
subcategory: "Service Networking"
description: |-
  Manages creating a private VPC connection to a service provider.
---</rdfs:comment>
  </owl:Class>
  <owl:DatatypeProperty rdf:about="http://example.org/onto/prop/google_service_networking_connection_deletion_policy">
    <rdfs:label>deletion_policy</rdfs:label>
    <rdfs:comment>When set to ABANDON, terraform will abandon management of the resource instead of deleting it. Prevents terraform apply failures with CloudSQL. Note: The resource will still exist.</rdfs:comment>
    <rdfs:domain rdf:resource="http://example.org/onto/class/google_service_networking_connection"/>
    <rdfs:range rdf:resource="http://www.w3.org/2001/XMLSchema#string"/>
  </owl:DatatypeProperty>
  <owl:DatatypeProperty rdf:about="http://example.org/onto/prop/google_service_networking_connection_id">
    <rdfs:label>id</rdfs:label>
    <rdfs:domain rdf:resource="http://example.org/onto/class/google_service_networking_connection"/>
    <rdfs:range rdf:resource="http://www.w3.org/2001/XMLSchema#string"/>
  </owl:DatatypeProperty>
  <owl:DatatypeProperty rdf:about="http://example.org/onto/prop/google_service_networking_connection_network">
    <rdfs:label>network</rdfs:label>
    <rdfs:comment>Name of VPC network connected with service producers using VPC peering.</rdfs:comment>
    <rdfs:domain rdf:resource="http://example.org/onto/class/google_service_networking_connection"/>
    <rdfs:range rdf:resource="http://www.w3.org/2001/XMLSchema#string"/>
  </owl:DatatypeProperty>
  <owl:DatatypeProperty rdf:about="http://example.org/onto/prop/google_service_networking_connection_peering">
    <rdfs:label>peering</rdfs:label>
    <rdfs:domain rdf:resource="http://example.org/onto/class/google_service_networking_connection"/>
    <rdfs:range rdf:resource="http://www.w3.org/2001/XMLSchema#string"/>
  </owl:DatatypeProperty>
  <owl:DatatypeProperty rdf:about="http://example.org/onto/prop/google_service_networking_connection_reserved_peering_ranges">
    <rdfs:label>reserved_peering_ranges</rdfs:label>
    <rdfs:comment>Named IP address range(s) of PEERING type reserved for this service provider. Note that invoking this method with a different range when connection is already established will not reallocate already provisioned service producer subnetworks.</rdfs:comment>
    <rdfs:domain rdf:resource="http://example.org/onto/class/google_service_networking_connection"/>
    <rdfs:range rdf:resource="http://www.w3.org/2001/XMLSchema#string"/>
  </owl:DatatypeProperty>
  <owl:DatatypeProperty rdf:about="http://example.org/onto/prop/google_service_networking_connection_service">
    <rdfs:label>service</rdfs:label>
    <rdfs:comment>Provider peering service that is managing peering connectivity for a service provider organization. For Google services that support this functionality it is 'servicenetworking.googleapis.com'.</rdfs:comment>
    <rdfs:domain rdf:resource="http://example.org/onto/class/google_service_networking_connection"/>
    <rdfs:range rdf:resource="http://www.w3.org/2001/XMLSchema#string"/>
  </owl:DatatypeProperty>
  <owl:DatatypeProperty rdf:about="http://example.org/onto/prop/google_service_networking_connection_update_on_creation_fail">
    <rdfs:label>update_on_creation_fail</rdfs:label>
    <rdfs:comment>When set to true, enforce an update of the reserved peering ranges on the existing service networking connection in case of a new connection creation failure.</rdfs:comment>
    <rdfs:domain rdf:resource="http://example.org/onto/class/google_service_networking_connection"/>
    <rdfs:range rdf:resource="http://www.w3.org/2001/XMLSchema#string"/>
  </owl:DatatypeProperty>
  <owl:DatatypeProperty rdf:about="http://example.org/onto/prop/google_service_networking_connection_create">
    <rdfs:label>create</rdfs:label>
    <rdfs:domain rdf:resource="http://example.org/onto/class/google_service_networking_connection"/>
    <rdfs:range rdf:resource="http://www.w3.org/2001/XMLSchema#string"/>
  </owl:DatatypeProperty>
  <owl:DatatypeProperty rdf:about="http://example.org/onto/prop/google_service_networking_connection_delete">
    <rdfs:label>delete</rdfs:label>
    <rdfs:domain rdf:resource="http://example.org/onto/class/google_service_networking_connection"/>
    <rdfs:range rdf:resource="http://www.w3.org/2001/XMLSchema#string"/>
  </owl:DatatypeProperty>
  <owl:DatatypeProperty rdf:about="http://example.org/onto/prop/google_service_networking_connection_update">
    <rdfs:label>update</rdfs:label>
    <rdfs:domain rdf:resource="http://example.org/onto/class/google_service_networking_connection"/>
    <rdfs:range rdf:resource="http://www.w3.org/2001/XMLSchema#string"/>
  </owl:DatatypeProperty>
</rdf:RDF>
