<?xml version="1.0" encoding="UTF-8"?>
<rdf:RDF
  xmlns:rdf="http://www.w3.org/1999/02/22-rdf-syntax-ns#"
  xmlns:rdfs="http://www.w3.org/2000/01/rdf-schema#"
  xmlns:owl="http://www.w3.org/2002/07/owl#"
  xmlns:xsd="http://www.w3.org/2001/XMLSchema#"
  xml:base="http://example.org/onto/">
  <owl:Class rdf:about="http://example.org/onto/class/google_workbench_instance">
    <rdfs:label>google_workbench_instance</rdfs:label>
    <rdfs:comment>#
#     ***     AUTO GENERATED CODE    ***    Type: MMv1     ***
#
# ----------------------------------------------------------------------------
#
#     This code is generated by Magic Modules using the following:
#
#     Configuration: https:#github.com/GoogleCloudPlatform/magic-modules/tree/main/mmv1/products/workbench/Instance.yaml
#     Template:      https:#github.com/GoogleCloudPlatform/magic-modules/tree/main/mmv1/templates/terraform/resource.html.markdown.tmpl
#
#     DO NOT EDIT this file directly. Any changes made to this file will be
#     overwritten during the next generation cycle.
#
# ----------------------------------------------------------------------------
subcategory: "Vertex AI Workbench"
description: |-
  A Workbench instance.
---</rdfs:comment>
  </owl:Class>
  <owl:DatatypeProperty rdf:about="http://example.org/onto/prop/google_workbench_instance_create_time">
    <rdfs:label>create_time</rdfs:label>
    <rdfs:comment>An RFC3339 timestamp in UTC time. This in the format of yyyy-MM-ddTHH:mm:ss.SSSZ.
The milliseconds portion (".SSS") is optional.</rdfs:comment>
    <rdfs:domain rdf:resource="http://example.org/onto/class/google_workbench_instance"/>
    <rdfs:range rdf:resource="http://www.w3.org/2001/XMLSchema#string"/>
  </owl:DatatypeProperty>
  <owl:DatatypeProperty rdf:about="http://example.org/onto/prop/google_workbench_instance_creator">
    <rdfs:label>creator</rdfs:label>
    <rdfs:comment>Output only. Email address of entity that sent original CreateInstance request.</rdfs:comment>
    <rdfs:domain rdf:resource="http://example.org/onto/class/google_workbench_instance"/>
    <rdfs:range rdf:resource="http://www.w3.org/2001/XMLSchema#string"/>
  </owl:DatatypeProperty>
  <owl:DatatypeProperty rdf:about="http://example.org/onto/prop/google_workbench_instance_desired_state">
    <rdfs:label>desired_state</rdfs:label>
    <rdfs:comment>Desired state of the Workbench Instance. Set this field to 'ACTIVE' to start the Instance, and 'STOPPED' to stop the Instance.</rdfs:comment>
    <rdfs:domain rdf:resource="http://example.org/onto/class/google_workbench_instance"/>
    <rdfs:range rdf:resource="http://www.w3.org/2001/XMLSchema#string"/>
  </owl:DatatypeProperty>
  <owl:DatatypeProperty rdf:about="http://example.org/onto/prop/google_workbench_instance_disable_proxy_access">
    <rdfs:label>disable_proxy_access</rdfs:label>
    <rdfs:comment>Optional. If true, the workbench instance will not register with the proxy.</rdfs:comment>
    <rdfs:domain rdf:resource="http://example.org/onto/class/google_workbench_instance"/>
    <rdfs:range rdf:resource="http://www.w3.org/2001/XMLSchema#string"/>
  </owl:DatatypeProperty>
  <owl:DatatypeProperty rdf:about="http://example.org/onto/prop/google_workbench_instance_effective_labels">
    <rdfs:label>effective_labels</rdfs:label>
    <rdfs:comment>All of labels (key/value pairs) present on the resource in GCP, including the labels configured through Terraform, other clients and services.</rdfs:comment>
    <rdfs:domain rdf:resource="http://example.org/onto/class/google_workbench_instance"/>
    <rdfs:range rdf:resource="http://www.w3.org/2001/XMLSchema#string"/>
  </owl:DatatypeProperty>
  <owl:DatatypeProperty rdf:about="http://example.org/onto/prop/google_workbench_instance_enable_managed_euc">
    <rdfs:label>enable_managed_euc</rdfs:label>
    <rdfs:comment>Flag to enable managed end user credentials for the instance.</rdfs:comment>
    <rdfs:domain rdf:resource="http://example.org/onto/class/google_workbench_instance"/>
    <rdfs:range rdf:resource="http://www.w3.org/2001/XMLSchema#string"/>
  </owl:DatatypeProperty>
  <owl:DatatypeProperty rdf:about="http://example.org/onto/prop/google_workbench_instance_enable_third_party_identity">
    <rdfs:label>enable_third_party_identity</rdfs:label>
    <rdfs:comment>Flag that specifies that a notebook can be accessed with third party
identity provider.</rdfs:comment>
    <rdfs:domain rdf:resource="http://example.org/onto/class/google_workbench_instance"/>
    <rdfs:range rdf:resource="http://www.w3.org/2001/XMLSchema#string"/>
  </owl:DatatypeProperty>
  <owl:DatatypeProperty rdf:about="http://example.org/onto/prop/google_workbench_instance_health_info">
    <rdfs:label>health_info</rdfs:label>
    <rdfs:comment>'Output only. Additional information about instance health. Example:
healthInfo": { "docker_proxy_agent_status": "1", "docker_status": "1", "jupyterlab_api_status":
"-1", "jupyterlab_status": "-1", "updated": "2020-10-18 09:40:03.573409" }'</rdfs:comment>
    <rdfs:domain rdf:resource="http://example.org/onto/class/google_workbench_instance"/>
    <rdfs:range rdf:resource="http://www.w3.org/2001/XMLSchema#string"/>
  </owl:DatatypeProperty>
  <owl:DatatypeProperty rdf:about="http://example.org/onto/prop/google_workbench_instance_health_state">
    <rdfs:label>health_state</rdfs:label>
    <rdfs:comment>Output only. Instance health_state.</rdfs:comment>
    <rdfs:domain rdf:resource="http://example.org/onto/class/google_workbench_instance"/>
    <rdfs:range rdf:resource="http://www.w3.org/2001/XMLSchema#string"/>
  </owl:DatatypeProperty>
  <owl:DatatypeProperty rdf:about="http://example.org/onto/prop/google_workbench_instance_id">
    <rdfs:label>id</rdfs:label>
    <rdfs:domain rdf:resource="http://example.org/onto/class/google_workbench_instance"/>
    <rdfs:range rdf:resource="http://www.w3.org/2001/XMLSchema#string"/>
  </owl:DatatypeProperty>
  <owl:DatatypeProperty rdf:about="http://example.org/onto/prop/google_workbench_instance_instance_id">
    <rdfs:label>instance_id</rdfs:label>
    <rdfs:comment>Required. User-defined unique ID of this instance.</rdfs:comment>
    <rdfs:domain rdf:resource="http://example.org/onto/class/google_workbench_instance"/>
    <rdfs:range rdf:resource="http://www.w3.org/2001/XMLSchema#string"/>
  </owl:DatatypeProperty>
  <owl:DatatypeProperty rdf:about="http://example.org/onto/prop/google_workbench_instance_instance_owners">
    <rdfs:label>instance_owners</rdfs:label>
    <rdfs:comment>'Optional. Input only. The owner of this instance after creation. Format:
'alias@example.com' Currently supports one owner only. If not specified, all of
the service account users of your VM instance''s service account can use the instance.
If specified, sets the access mode to 'Single user'. For more details, see
https://cloud.google.com/vertex-ai/docs/workbench/instances/manage-access-jupyterlab'</rdfs:comment>
    <rdfs:domain rdf:resource="http://example.org/onto/class/google_workbench_instance"/>
    <rdfs:range rdf:resource="http://www.w3.org/2001/XMLSchema#string"/>
  </owl:DatatypeProperty>
  <owl:DatatypeProperty rdf:about="http://example.org/onto/prop/google_workbench_instance_labels">
    <rdfs:label>labels</rdfs:label>
    <rdfs:comment>Optional. Labels to apply to this instance. These can be later modified
by the UpdateInstance method.


**Note**: This field is non-authoritative, and will only manage the labels present in your configuration.
Please refer to the field 'effective_labels' for all of the labels present on the resource.</rdfs:comment>
    <rdfs:domain rdf:resource="http://example.org/onto/class/google_workbench_instance"/>
    <rdfs:range rdf:resource="http://www.w3.org/2001/XMLSchema#string"/>
  </owl:DatatypeProperty>
  <owl:DatatypeProperty rdf:about="http://example.org/onto/prop/google_workbench_instance_location">
    <rdfs:label>location</rdfs:label>
    <rdfs:comment>Part of 'parent'. See documentation of 'projectsId'.</rdfs:comment>
    <rdfs:domain rdf:resource="http://example.org/onto/class/google_workbench_instance"/>
    <rdfs:range rdf:resource="http://www.w3.org/2001/XMLSchema#string"/>
  </owl:DatatypeProperty>
  <owl:DatatypeProperty rdf:about="http://example.org/onto/prop/google_workbench_instance_name">
    <rdfs:label>name</rdfs:label>
    <rdfs:comment>The name of this workbench instance. Format: 'projects/{project_id}/locations/{location}/instances/{instance_id}'</rdfs:comment>
    <rdfs:domain rdf:resource="http://example.org/onto/class/google_workbench_instance"/>
    <rdfs:range rdf:resource="http://www.w3.org/2001/XMLSchema#string"/>
  </owl:DatatypeProperty>
  <owl:DatatypeProperty rdf:about="http://example.org/onto/prop/google_workbench_instance_project">
    <rdfs:label>project</rdfs:label>
    <rdfs:domain rdf:resource="http://example.org/onto/class/google_workbench_instance"/>
    <rdfs:range rdf:resource="http://www.w3.org/2001/XMLSchema#string"/>
  </owl:DatatypeProperty>
  <owl:DatatypeProperty rdf:about="http://example.org/onto/prop/google_workbench_instance_proxy_uri">
    <rdfs:label>proxy_uri</rdfs:label>
    <rdfs:comment>Output only. The proxy endpoint that is used to access the Jupyter notebook.</rdfs:comment>
    <rdfs:domain rdf:resource="http://example.org/onto/class/google_workbench_instance"/>
    <rdfs:range rdf:resource="http://www.w3.org/2001/XMLSchema#string"/>
  </owl:DatatypeProperty>
  <owl:DatatypeProperty rdf:about="http://example.org/onto/prop/google_workbench_instance_state">
    <rdfs:label>state</rdfs:label>
    <rdfs:comment>Output only. The state of this instance.</rdfs:comment>
    <rdfs:domain rdf:resource="http://example.org/onto/class/google_workbench_instance"/>
    <rdfs:range rdf:resource="http://www.w3.org/2001/XMLSchema#string"/>
  </owl:DatatypeProperty>
  <owl:DatatypeProperty rdf:about="http://example.org/onto/prop/google_workbench_instance_terraform_labels">
    <rdfs:label>terraform_labels</rdfs:label>
    <rdfs:comment>The combination of labels configured directly on the resource
 and default labels configured on the provider.</rdfs:comment>
    <rdfs:domain rdf:resource="http://example.org/onto/class/google_workbench_instance"/>
    <rdfs:range rdf:resource="http://www.w3.org/2001/XMLSchema#string"/>
  </owl:DatatypeProperty>
  <owl:DatatypeProperty rdf:about="http://example.org/onto/prop/google_workbench_instance_update_time">
    <rdfs:label>update_time</rdfs:label>
    <rdfs:comment>An RFC3339 timestamp in UTC time. This in the format of yyyy-MM-ddTHH:mm:ss.SSSZ.
The milliseconds portion (".SSS") is optional.</rdfs:comment>
    <rdfs:domain rdf:resource="http://example.org/onto/class/google_workbench_instance"/>
    <rdfs:range rdf:resource="http://www.w3.org/2001/XMLSchema#string"/>
  </owl:DatatypeProperty>
  <owl:DatatypeProperty rdf:about="http://example.org/onto/prop/google_workbench_instance_upgrade_history">
    <rdfs:label>upgrade_history</rdfs:label>
    <rdfs:comment>Output only. The upgrade history of this instance.</rdfs:comment>
    <rdfs:domain rdf:resource="http://example.org/onto/class/google_workbench_instance"/>
    <rdfs:range rdf:resource="http://www.w3.org/2001/XMLSchema#string"/>
  </owl:DatatypeProperty>
  <owl:DatatypeProperty rdf:about="http://example.org/onto/prop/google_workbench_instance_disable_public_ip">
    <rdfs:label>disable_public_ip</rdfs:label>
    <rdfs:comment>Optional. If true, no external IP will be assigned to this VM instance.</rdfs:comment>
    <rdfs:domain rdf:resource="http://example.org/onto/class/google_workbench_instance"/>
    <rdfs:range rdf:resource="http://www.w3.org/2001/XMLSchema#string"/>
  </owl:DatatypeProperty>
  <owl:DatatypeProperty rdf:about="http://example.org/onto/prop/google_workbench_instance_enable_ip_forwarding">
    <rdfs:label>enable_ip_forwarding</rdfs:label>
    <rdfs:comment>Optional. Flag to enable ip forwarding or not, default false/off.
https://cloud.google.com/vpc/docs/using-routes#canipforward</rdfs:comment>
    <rdfs:domain rdf:resource="http://example.org/onto/class/google_workbench_instance"/>
    <rdfs:range rdf:resource="http://www.w3.org/2001/XMLSchema#string"/>
  </owl:DatatypeProperty>
  <owl:DatatypeProperty rdf:about="http://example.org/onto/prop/google_workbench_instance_machine_type">
    <rdfs:label>machine_type</rdfs:label>
    <rdfs:comment>Optional. The machine type of the VM instance. https://cloud.google.com/compute/docs/machine-resource</rdfs:comment>
    <rdfs:domain rdf:resource="http://example.org/onto/class/google_workbench_instance"/>
    <rdfs:range rdf:resource="http://www.w3.org/2001/XMLSchema#string"/>
  </owl:DatatypeProperty>
  <owl:DatatypeProperty rdf:about="http://example.org/onto/prop/google_workbench_instance_metadata">
    <rdfs:label>metadata</rdfs:label>
    <rdfs:comment>Optional. Custom metadata to apply to this instance.</rdfs:comment>
    <rdfs:domain rdf:resource="http://example.org/onto/class/google_workbench_instance"/>
    <rdfs:range rdf:resource="http://www.w3.org/2001/XMLSchema#string"/>
  </owl:DatatypeProperty>
  <owl:DatatypeProperty rdf:about="http://example.org/onto/prop/google_workbench_instance_tags">
    <rdfs:label>tags</rdfs:label>
    <rdfs:comment>Optional. The Compute Engine tags to add to instance (see [Tagging
instances](https://cloud.google.com/compute/docs/label-or-tag-resources#tags)).</rdfs:comment>
    <rdfs:domain rdf:resource="http://example.org/onto/class/google_workbench_instance"/>
    <rdfs:range rdf:resource="http://www.w3.org/2001/XMLSchema#string"/>
  </owl:DatatypeProperty>
  <owl:DatatypeProperty rdf:about="http://example.org/onto/prop/google_workbench_instance_core_count">
    <rdfs:label>core_count</rdfs:label>
    <rdfs:comment>Optional. Count of cores of this accelerator.</rdfs:comment>
    <rdfs:domain rdf:resource="http://example.org/onto/class/google_workbench_instance"/>
    <rdfs:range rdf:resource="http://www.w3.org/2001/XMLSchema#string"/>
  </owl:DatatypeProperty>
  <owl:DatatypeProperty rdf:about="http://example.org/onto/prop/google_workbench_instance_type">
    <rdfs:label>type</rdfs:label>
    <rdfs:comment>Optional. Type of this accelerator. Possible values: ["NVIDIA_TESLA_P100", "NVIDIA_TESLA_V100", "NVIDIA_TESLA_P4", "NVIDIA_TESLA_T4", "NVIDIA_TESLA_A100", "NVIDIA_A100_80GB", "NVIDIA_L4", "NVIDIA_TESLA_T4_VWS", "NVIDIA_TESLA_P100_VWS", "NVIDIA_TESLA_P4_VWS"]</rdfs:comment>
    <rdfs:domain rdf:resource="http://example.org/onto/class/google_workbench_instance"/>
    <rdfs:range rdf:resource="http://www.w3.org/2001/XMLSchema#string"/>
  </owl:DatatypeProperty>
  <owl:DatatypeProperty rdf:about="http://example.org/onto/prop/google_workbench_instance_disk_encryption">
    <rdfs:label>disk_encryption</rdfs:label>
    <rdfs:comment>Optional. Input only. Disk encryption method used on the boot and
data disks, defaults to GMEK. Possible values: ["GMEK", "CMEK"]</rdfs:comment>
    <rdfs:domain rdf:resource="http://example.org/onto/class/google_workbench_instance"/>
    <rdfs:range rdf:resource="http://www.w3.org/2001/XMLSchema#string"/>
  </owl:DatatypeProperty>
  <owl:DatatypeProperty rdf:about="http://example.org/onto/prop/google_workbench_instance_disk_size_gb">
    <rdfs:label>disk_size_gb</rdfs:label>
    <rdfs:comment>Optional. The size of the boot disk in GB attached to this instance,
up to a maximum of 64000 GB (64 TB). If not specified, this defaults to the
recommended value of 150GB.</rdfs:comment>
    <rdfs:domain rdf:resource="http://example.org/onto/class/google_workbench_instance"/>
    <rdfs:range rdf:resource="http://www.w3.org/2001/XMLSchema#string"/>
  </owl:DatatypeProperty>
  <owl:DatatypeProperty rdf:about="http://example.org/onto/prop/google_workbench_instance_disk_type">
    <rdfs:label>disk_type</rdfs:label>
    <rdfs:comment>Optional. Indicates the type of the disk. Possible values: ["PD_STANDARD", "PD_SSD", "PD_BALANCED", "PD_EXTREME"]</rdfs:comment>
    <rdfs:domain rdf:resource="http://example.org/onto/class/google_workbench_instance"/>
    <rdfs:range rdf:resource="http://www.w3.org/2001/XMLSchema#string"/>
  </owl:DatatypeProperty>
  <owl:DatatypeProperty rdf:about="http://example.org/onto/prop/google_workbench_instance_kms_key">
    <rdfs:label>kms_key</rdfs:label>
    <rdfs:comment>'Optional. The KMS key used to encrypt the disks, only
applicable if disk_encryption is CMEK. Format: 'projects/{project_id}/locations/{location}/keyRings/{key_ring_id}/cryptoKeys/{key_id}'
Learn more about using your own encryption keys.'</rdfs:comment>
    <rdfs:domain rdf:resource="http://example.org/onto/class/google_workbench_instance"/>
    <rdfs:range rdf:resource="http://www.w3.org/2001/XMLSchema#string"/>
  </owl:DatatypeProperty>
  <owl:DatatypeProperty rdf:about="http://example.org/onto/prop/google_workbench_instance_confidential_instance_type">
    <rdfs:label>confidential_instance_type</rdfs:label>
    <rdfs:comment>Defines the type of technology used by the confidential instance. Possible values: ["SEV"]</rdfs:comment>
    <rdfs:domain rdf:resource="http://example.org/onto/class/google_workbench_instance"/>
    <rdfs:range rdf:resource="http://www.w3.org/2001/XMLSchema#string"/>
  </owl:DatatypeProperty>
  <owl:DatatypeProperty rdf:about="http://example.org/onto/prop/google_workbench_instance_repository">
    <rdfs:label>repository</rdfs:label>
    <rdfs:comment>The path to the container image repository.
For example: gcr.io/{project_id}/{imageName}</rdfs:comment>
    <rdfs:domain rdf:resource="http://example.org/onto/class/google_workbench_instance"/>
    <rdfs:range rdf:resource="http://www.w3.org/2001/XMLSchema#string"/>
  </owl:DatatypeProperty>
  <owl:DatatypeProperty rdf:about="http://example.org/onto/prop/google_workbench_instance_tag">
    <rdfs:label>tag</rdfs:label>
    <rdfs:comment>The tag of the container image. If not specified, this defaults to the latest tag.</rdfs:comment>
    <rdfs:domain rdf:resource="http://example.org/onto/class/google_workbench_instance"/>
    <rdfs:range rdf:resource="http://www.w3.org/2001/XMLSchema#string"/>
  </owl:DatatypeProperty>
  <owl:DatatypeProperty rdf:about="http://example.org/onto/prop/google_workbench_instance_disk_encryption">
    <rdfs:label>disk_encryption</rdfs:label>
    <rdfs:comment>Optional. Input only. Disk encryption method used on the boot
and data disks, defaults to GMEK. Possible values: ["GMEK", "CMEK"]</rdfs:comment>
    <rdfs:domain rdf:resource="http://example.org/onto/class/google_workbench_instance"/>
    <rdfs:range rdf:resource="http://www.w3.org/2001/XMLSchema#string"/>
  </owl:DatatypeProperty>
  <owl:DatatypeProperty rdf:about="http://example.org/onto/prop/google_workbench_instance_disk_size_gb">
    <rdfs:label>disk_size_gb</rdfs:label>
    <rdfs:comment>Optional. The size of the disk in GB attached to this VM instance,
up to a maximum of 64000 GB (64 TB). If not specified, this defaults to
100.</rdfs:comment>
    <rdfs:domain rdf:resource="http://example.org/onto/class/google_workbench_instance"/>
    <rdfs:range rdf:resource="http://www.w3.org/2001/XMLSchema#string"/>
  </owl:DatatypeProperty>
  <owl:DatatypeProperty rdf:about="http://example.org/onto/prop/google_workbench_instance_disk_type">
    <rdfs:label>disk_type</rdfs:label>
    <rdfs:comment>Optional. Input only. Indicates the type of the disk. Possible values: ["PD_STANDARD", "PD_SSD", "PD_BALANCED", "PD_EXTREME"]</rdfs:comment>
    <rdfs:domain rdf:resource="http://example.org/onto/class/google_workbench_instance"/>
    <rdfs:range rdf:resource="http://www.w3.org/2001/XMLSchema#string"/>
  </owl:DatatypeProperty>
  <owl:DatatypeProperty rdf:about="http://example.org/onto/prop/google_workbench_instance_kms_key">
    <rdfs:label>kms_key</rdfs:label>
    <rdfs:comment>'Optional. The KMS key used to encrypt the disks,
only applicable if disk_encryption is CMEK. Format: 'projects/{project_id}/locations/{location}/keyRings/{key_ring_id}/cryptoKeys/{key_id}'
Learn more about using your own encryption keys.'</rdfs:comment>
    <rdfs:domain rdf:resource="http://example.org/onto/class/google_workbench_instance"/>
    <rdfs:range rdf:resource="http://www.w3.org/2001/XMLSchema#string"/>
  </owl:DatatypeProperty>
  <owl:DatatypeProperty rdf:about="http://example.org/onto/prop/google_workbench_instance_network">
    <rdfs:label>network</rdfs:label>
    <rdfs:comment>Optional. The name of the VPC that this VM instance is in.</rdfs:comment>
    <rdfs:domain rdf:resource="http://example.org/onto/class/google_workbench_instance"/>
    <rdfs:range rdf:resource="http://www.w3.org/2001/XMLSchema#string"/>
  </owl:DatatypeProperty>
  <owl:DatatypeProperty rdf:about="http://example.org/onto/prop/google_workbench_instance_nic_type">
    <rdfs:label>nic_type</rdfs:label>
    <rdfs:comment>Optional. The type of vNIC to be used on this interface. This
may be gVNIC or VirtioNet. Possible values: ["VIRTIO_NET", "GVNIC"]</rdfs:comment>
    <rdfs:domain rdf:resource="http://example.org/onto/class/google_workbench_instance"/>
    <rdfs:range rdf:resource="http://www.w3.org/2001/XMLSchema#string"/>
  </owl:DatatypeProperty>
  <owl:DatatypeProperty rdf:about="http://example.org/onto/prop/google_workbench_instance_subnet">
    <rdfs:label>subnet</rdfs:label>
    <rdfs:comment>Optional. The name of the subnet that this VM instance is in.</rdfs:comment>
    <rdfs:domain rdf:resource="http://example.org/onto/class/google_workbench_instance"/>
    <rdfs:range rdf:resource="http://www.w3.org/2001/XMLSchema#string"/>
  </owl:DatatypeProperty>
  <owl:DatatypeProperty rdf:about="http://example.org/onto/prop/google_workbench_instance_external_ip">
    <rdfs:label>external_ip</rdfs:label>
    <rdfs:comment>An external IP address associated with this instance. Specify an unused
static external IP address available to the project or leave this field
undefined to use an IP from a shared ephemeral IP address pool. If you
specify a static external IP address, it must live in the same region as
the zone of the instance.</rdfs:comment>
    <rdfs:domain rdf:resource="http://example.org/onto/class/google_workbench_instance"/>
    <rdfs:range rdf:resource="http://www.w3.org/2001/XMLSchema#string"/>
  </owl:DatatypeProperty>
  <owl:DatatypeProperty rdf:about="http://example.org/onto/prop/google_workbench_instance_consume_reservation_type">
    <rdfs:label>consume_reservation_type</rdfs:label>
    <rdfs:comment>Specifies the type of reservation from which this instance can consume resources:
RESERVATION_ANY (default), RESERVATION_SPECIFIC, or RESERVATION_NONE. Possible values: ["RESERVATION_NONE", "RESERVATION_ANY", "RESERVATION_SPECIFIC"]</rdfs:comment>
    <rdfs:domain rdf:resource="http://example.org/onto/class/google_workbench_instance"/>
    <rdfs:range rdf:resource="http://www.w3.org/2001/XMLSchema#string"/>
  </owl:DatatypeProperty>
  <owl:DatatypeProperty rdf:about="http://example.org/onto/prop/google_workbench_instance_key">
    <rdfs:label>key</rdfs:label>
    <rdfs:comment>Corresponds to the label key of a reservation resource. To target a
RESERVATION_SPECIFIC by name, use compute.googleapis.com/reservation-name
as the key and specify the name of your reservation as its value.</rdfs:comment>
    <rdfs:domain rdf:resource="http://example.org/onto/class/google_workbench_instance"/>
    <rdfs:range rdf:resource="http://www.w3.org/2001/XMLSchema#string"/>
  </owl:DatatypeProperty>
  <owl:DatatypeProperty rdf:about="http://example.org/onto/prop/google_workbench_instance_values">
    <rdfs:label>values</rdfs:label>
    <rdfs:comment>Corresponds to the label values of a reservation resource. This can be
either a name to a reservation in the same project or
"projects/different-project/reservations/some-reservation-name"
to target a shared reservation in the same zone but in a different project.</rdfs:comment>
    <rdfs:domain rdf:resource="http://example.org/onto/class/google_workbench_instance"/>
    <rdfs:range rdf:resource="http://www.w3.org/2001/XMLSchema#string"/>
  </owl:DatatypeProperty>
  <owl:DatatypeProperty rdf:about="http://example.org/onto/prop/google_workbench_instance_email">
    <rdfs:label>email</rdfs:label>
    <rdfs:comment>Optional. Email address of the service account.</rdfs:comment>
    <rdfs:domain rdf:resource="http://example.org/onto/class/google_workbench_instance"/>
    <rdfs:range rdf:resource="http://www.w3.org/2001/XMLSchema#string"/>
  </owl:DatatypeProperty>
  <owl:DatatypeProperty rdf:about="http://example.org/onto/prop/google_workbench_instance_scopes">
    <rdfs:label>scopes</rdfs:label>
    <rdfs:comment>Output only. The list of scopes to be made available for this
service account. Set by the CLH to https://www.googleapis.com/auth/cloud-platform</rdfs:comment>
    <rdfs:domain rdf:resource="http://example.org/onto/class/google_workbench_instance"/>
    <rdfs:range rdf:resource="http://www.w3.org/2001/XMLSchema#string"/>
  </owl:DatatypeProperty>
  <owl:DatatypeProperty rdf:about="http://example.org/onto/prop/google_workbench_instance_enable_integrity_monitoring">
    <rdfs:label>enable_integrity_monitoring</rdfs:label>
    <rdfs:comment>Optional. Defines whether the VM instance has integrity monitoring
enabled. Enables monitoring and attestation of the boot integrity of the VM
instance. The attestation is performed against the integrity policy baseline.
This baseline is initially derived from the implicitly trusted boot image
when the VM instance is created. Enabled by default.</rdfs:comment>
    <rdfs:domain rdf:resource="http://example.org/onto/class/google_workbench_instance"/>
    <rdfs:range rdf:resource="http://www.w3.org/2001/XMLSchema#string"/>
  </owl:DatatypeProperty>
  <owl:DatatypeProperty rdf:about="http://example.org/onto/prop/google_workbench_instance_enable_secure_boot">
    <rdfs:label>enable_secure_boot</rdfs:label>
    <rdfs:comment>Optional. Defines whether the VM instance has Secure Boot enabled.
Secure Boot helps ensure that the system only runs authentic software by verifying
the digital signature of all boot components, and halting the boot process
if signature verification fails. Disabled by default.</rdfs:comment>
    <rdfs:domain rdf:resource="http://example.org/onto/class/google_workbench_instance"/>
    <rdfs:range rdf:resource="http://www.w3.org/2001/XMLSchema#string"/>
  </owl:DatatypeProperty>
  <owl:DatatypeProperty rdf:about="http://example.org/onto/prop/google_workbench_instance_enable_vtpm">
    <rdfs:label>enable_vtpm</rdfs:label>
    <rdfs:comment>Optional. Defines whether the VM instance has the vTPM enabled.
Enabled by default.</rdfs:comment>
    <rdfs:domain rdf:resource="http://example.org/onto/class/google_workbench_instance"/>
    <rdfs:range rdf:resource="http://www.w3.org/2001/XMLSchema#string"/>
  </owl:DatatypeProperty>
  <owl:DatatypeProperty rdf:about="http://example.org/onto/prop/google_workbench_instance_family">
    <rdfs:label>family</rdfs:label>
    <rdfs:comment>Optional. Use this VM image family to find the image; the newest
image in this family will be used.</rdfs:comment>
    <rdfs:domain rdf:resource="http://example.org/onto/class/google_workbench_instance"/>
    <rdfs:range rdf:resource="http://www.w3.org/2001/XMLSchema#string"/>
  </owl:DatatypeProperty>
  <owl:DatatypeProperty rdf:about="http://example.org/onto/prop/google_workbench_instance_name">
    <rdfs:label>name</rdfs:label>
    <rdfs:comment>Optional. Use VM image name to find the image.</rdfs:comment>
    <rdfs:domain rdf:resource="http://example.org/onto/class/google_workbench_instance"/>
    <rdfs:range rdf:resource="http://www.w3.org/2001/XMLSchema#string"/>
  </owl:DatatypeProperty>
  <owl:DatatypeProperty rdf:about="http://example.org/onto/prop/google_workbench_instance_project">
    <rdfs:label>project</rdfs:label>
    <rdfs:comment>The name of the Google Cloud project that this VM image belongs to.
Format: {project_id}</rdfs:comment>
    <rdfs:domain rdf:resource="http://example.org/onto/class/google_workbench_instance"/>
    <rdfs:range rdf:resource="http://www.w3.org/2001/XMLSchema#string"/>
  </owl:DatatypeProperty>
  <owl:DatatypeProperty rdf:about="http://example.org/onto/prop/google_workbench_instance_create">
    <rdfs:label>create</rdfs:label>
    <rdfs:domain rdf:resource="http://example.org/onto/class/google_workbench_instance"/>
    <rdfs:range rdf:resource="http://www.w3.org/2001/XMLSchema#string"/>
  </owl:DatatypeProperty>
  <owl:DatatypeProperty rdf:about="http://example.org/onto/prop/google_workbench_instance_delete">
    <rdfs:label>delete</rdfs:label>
    <rdfs:domain rdf:resource="http://example.org/onto/class/google_workbench_instance"/>
    <rdfs:range rdf:resource="http://www.w3.org/2001/XMLSchema#string"/>
  </owl:DatatypeProperty>
  <owl:DatatypeProperty rdf:about="http://example.org/onto/prop/google_workbench_instance_update">
    <rdfs:label>update</rdfs:label>
    <rdfs:domain rdf:resource="http://example.org/onto/class/google_workbench_instance"/>
    <rdfs:range rdf:resource="http://www.w3.org/2001/XMLSchema#string"/>
  </owl:DatatypeProperty>
</rdf:RDF>
