<?xml version="1.0" encoding="UTF-8"?>
<rdf:RDF
  xmlns:rdf="http://www.w3.org/1999/02/22-rdf-syntax-ns#"
  xmlns:rdfs="http://www.w3.org/2000/01/rdf-schema#"
  xmlns:owl="http://www.w3.org/2002/07/owl#"
  xmlns:xsd="http://www.w3.org/2001/XMLSchema#"
  xml:base="http://example.org/onto/">
  <owl:Class rdf:about="http://example.org/onto/class/google_chronicle_data_access_scope">
    <rdfs:label>google_chronicle_data_access_scope</rdfs:label>
    <rdfs:comment>#
#     ***     AUTO GENERATED CODE    ***    Type: MMv1     ***
#
# ----------------------------------------------------------------------------
#
#     This code is generated by Magic Modules using the following:
#
#     Configuration: https:#github.com/GoogleCloudPlatform/magic-modules/tree/main/mmv1/products/chronicle/DataAccessScope.yaml
#     Template:      https:#github.com/GoogleCloudPlatform/magic-modules/tree/main/mmv1/templates/terraform/resource.html.markdown.tmpl
#
#     DO NOT EDIT this file directly. Any changes made to this file will be
#     overwritten during the next generation cycle.
#
# ----------------------------------------------------------------------------
subcategory: "Chronicle"
description: |-
  A DataAccessScope is a boolean expression of data access labels used to restrict access to data for users.
---</rdfs:comment>
  </owl:Class>
  <owl:DatatypeProperty rdf:about="http://example.org/onto/prop/google_chronicle_data_access_scope_allow_all">
    <rdfs:label>allow_all</rdfs:label>
    <rdfs:comment>Optional. Whether or not the scope allows all labels, allow_all and
allowed_data_access_labels are mutually exclusive and one of them must be
present. denied_data_access_labels can still be used along with allow_all.
When combined with denied_data_access_labels, access will be granted to all
data that doesn't have labels mentioned in denied_data_access_labels. E.g.:
A customer with scope with denied labels A and B and allow_all will be able
to see all data except data labeled with A and data labeled with B and data
with labels A and B.</rdfs:comment>
    <rdfs:domain rdf:resource="http://example.org/onto/class/google_chronicle_data_access_scope"/>
    <rdfs:range rdf:resource="http://www.w3.org/2001/XMLSchema#string"/>
  </owl:DatatypeProperty>
  <owl:DatatypeProperty rdf:about="http://example.org/onto/prop/google_chronicle_data_access_scope_author">
    <rdfs:label>author</rdfs:label>
    <rdfs:comment>Output only. The user who created the data access scope.</rdfs:comment>
    <rdfs:domain rdf:resource="http://example.org/onto/class/google_chronicle_data_access_scope"/>
    <rdfs:range rdf:resource="http://www.w3.org/2001/XMLSchema#string"/>
  </owl:DatatypeProperty>
  <owl:DatatypeProperty rdf:about="http://example.org/onto/prop/google_chronicle_data_access_scope_create_time">
    <rdfs:label>create_time</rdfs:label>
    <rdfs:comment>Output only. The time at which the data access scope was created.</rdfs:comment>
    <rdfs:domain rdf:resource="http://example.org/onto/class/google_chronicle_data_access_scope"/>
    <rdfs:range rdf:resource="http://www.w3.org/2001/XMLSchema#string"/>
  </owl:DatatypeProperty>
  <owl:DatatypeProperty rdf:about="http://example.org/onto/prop/google_chronicle_data_access_scope_data_access_scope_id">
    <rdfs:label>data_access_scope_id</rdfs:label>
    <rdfs:comment>Required. The user provided scope id which will become the last part of the name
of the scope resource.
Needs to be compliant with https://google.aip.dev/122</rdfs:comment>
    <rdfs:domain rdf:resource="http://example.org/onto/class/google_chronicle_data_access_scope"/>
    <rdfs:range rdf:resource="http://www.w3.org/2001/XMLSchema#string"/>
  </owl:DatatypeProperty>
  <owl:DatatypeProperty rdf:about="http://example.org/onto/prop/google_chronicle_data_access_scope_description">
    <rdfs:label>description</rdfs:label>
    <rdfs:comment>Optional. A description of the data access scope for a human reader.</rdfs:comment>
    <rdfs:domain rdf:resource="http://example.org/onto/class/google_chronicle_data_access_scope"/>
    <rdfs:range rdf:resource="http://www.w3.org/2001/XMLSchema#string"/>
  </owl:DatatypeProperty>
  <owl:DatatypeProperty rdf:about="http://example.org/onto/prop/google_chronicle_data_access_scope_display_name">
    <rdfs:label>display_name</rdfs:label>
    <rdfs:comment>Output only. The name to be used for display to customers of the data access scope.</rdfs:comment>
    <rdfs:domain rdf:resource="http://example.org/onto/class/google_chronicle_data_access_scope"/>
    <rdfs:range rdf:resource="http://www.w3.org/2001/XMLSchema#string"/>
  </owl:DatatypeProperty>
  <owl:DatatypeProperty rdf:about="http://example.org/onto/prop/google_chronicle_data_access_scope_id">
    <rdfs:label>id</rdfs:label>
    <rdfs:domain rdf:resource="http://example.org/onto/class/google_chronicle_data_access_scope"/>
    <rdfs:range rdf:resource="http://www.w3.org/2001/XMLSchema#string"/>
  </owl:DatatypeProperty>
  <owl:DatatypeProperty rdf:about="http://example.org/onto/prop/google_chronicle_data_access_scope_instance">
    <rdfs:label>instance</rdfs:label>
    <rdfs:comment>The unique identifier for the Chronicle instance, which is the same as the customer ID.</rdfs:comment>
    <rdfs:domain rdf:resource="http://example.org/onto/class/google_chronicle_data_access_scope"/>
    <rdfs:range rdf:resource="http://www.w3.org/2001/XMLSchema#string"/>
  </owl:DatatypeProperty>
  <owl:DatatypeProperty rdf:about="http://example.org/onto/prop/google_chronicle_data_access_scope_last_editor">
    <rdfs:label>last_editor</rdfs:label>
    <rdfs:comment>Output only. The user who last updated the data access scope.</rdfs:comment>
    <rdfs:domain rdf:resource="http://example.org/onto/class/google_chronicle_data_access_scope"/>
    <rdfs:range rdf:resource="http://www.w3.org/2001/XMLSchema#string"/>
  </owl:DatatypeProperty>
  <owl:DatatypeProperty rdf:about="http://example.org/onto/prop/google_chronicle_data_access_scope_location">
    <rdfs:label>location</rdfs:label>
    <rdfs:comment>The location of the resource. This is the geographical region where the Chronicle instance resides, such as "us" or "europe-west2".</rdfs:comment>
    <rdfs:domain rdf:resource="http://example.org/onto/class/google_chronicle_data_access_scope"/>
    <rdfs:range rdf:resource="http://www.w3.org/2001/XMLSchema#string"/>
  </owl:DatatypeProperty>
  <owl:DatatypeProperty rdf:about="http://example.org/onto/prop/google_chronicle_data_access_scope_name">
    <rdfs:label>name</rdfs:label>
    <rdfs:comment>The unique full name of the data access scope. This unique identifier is generated using values provided for the URL parameters.
Format:
projects/{project}/locations/{location}/instances/{instance}/dataAccessScopes/{data_access_scope_id}</rdfs:comment>
    <rdfs:domain rdf:resource="http://example.org/onto/class/google_chronicle_data_access_scope"/>
    <rdfs:range rdf:resource="http://www.w3.org/2001/XMLSchema#string"/>
  </owl:DatatypeProperty>
  <owl:DatatypeProperty rdf:about="http://example.org/onto/prop/google_chronicle_data_access_scope_project">
    <rdfs:label>project</rdfs:label>
    <rdfs:domain rdf:resource="http://example.org/onto/class/google_chronicle_data_access_scope"/>
    <rdfs:range rdf:resource="http://www.w3.org/2001/XMLSchema#string"/>
  </owl:DatatypeProperty>
  <owl:DatatypeProperty rdf:about="http://example.org/onto/prop/google_chronicle_data_access_scope_update_time">
    <rdfs:label>update_time</rdfs:label>
    <rdfs:comment>Output only. The time at which the data access scope was last updated.</rdfs:comment>
    <rdfs:domain rdf:resource="http://example.org/onto/class/google_chronicle_data_access_scope"/>
    <rdfs:range rdf:resource="http://www.w3.org/2001/XMLSchema#string"/>
  </owl:DatatypeProperty>
  <owl:DatatypeProperty rdf:about="http://example.org/onto/prop/google_chronicle_data_access_scope_asset_namespace">
    <rdfs:label>asset_namespace</rdfs:label>
    <rdfs:comment>The asset namespace configured in the forwarder
of the customer's events.</rdfs:comment>
    <rdfs:domain rdf:resource="http://example.org/onto/class/google_chronicle_data_access_scope"/>
    <rdfs:range rdf:resource="http://www.w3.org/2001/XMLSchema#string"/>
  </owl:DatatypeProperty>
  <owl:DatatypeProperty rdf:about="http://example.org/onto/prop/google_chronicle_data_access_scope_data_access_label">
    <rdfs:label>data_access_label</rdfs:label>
    <rdfs:comment>The name of the data access label.</rdfs:comment>
    <rdfs:domain rdf:resource="http://example.org/onto/class/google_chronicle_data_access_scope"/>
    <rdfs:range rdf:resource="http://www.w3.org/2001/XMLSchema#string"/>
  </owl:DatatypeProperty>
  <owl:DatatypeProperty rdf:about="http://example.org/onto/prop/google_chronicle_data_access_scope_display_name">
    <rdfs:label>display_name</rdfs:label>
    <rdfs:comment>Output only. The display name of the label.
Data access label and log types's name
will match the display name of the resource.
The asset namespace will match the namespace itself.
The ingestion key value pair will match the key of the tuple.</rdfs:comment>
    <rdfs:domain rdf:resource="http://example.org/onto/class/google_chronicle_data_access_scope"/>
    <rdfs:range rdf:resource="http://www.w3.org/2001/XMLSchema#string"/>
  </owl:DatatypeProperty>
  <owl:DatatypeProperty rdf:about="http://example.org/onto/prop/google_chronicle_data_access_scope_log_type">
    <rdfs:label>log_type</rdfs:label>
    <rdfs:comment>The name of the log type.</rdfs:comment>
    <rdfs:domain rdf:resource="http://example.org/onto/class/google_chronicle_data_access_scope"/>
    <rdfs:range rdf:resource="http://www.w3.org/2001/XMLSchema#string"/>
  </owl:DatatypeProperty>
  <owl:DatatypeProperty rdf:about="http://example.org/onto/prop/google_chronicle_data_access_scope_ingestion_label_key">
    <rdfs:label>ingestion_label_key</rdfs:label>
    <rdfs:comment>Required. The key of the ingestion label. Always required.</rdfs:comment>
    <rdfs:domain rdf:resource="http://example.org/onto/class/google_chronicle_data_access_scope"/>
    <rdfs:range rdf:resource="http://www.w3.org/2001/XMLSchema#string"/>
  </owl:DatatypeProperty>
  <owl:DatatypeProperty rdf:about="http://example.org/onto/prop/google_chronicle_data_access_scope_ingestion_label_value">
    <rdfs:label>ingestion_label_value</rdfs:label>
    <rdfs:comment>Optional. The value of the ingestion label. Optional. An object
with no provided value and some key provided would match
against the given key and ANY value.</rdfs:comment>
    <rdfs:domain rdf:resource="http://example.org/onto/class/google_chronicle_data_access_scope"/>
    <rdfs:range rdf:resource="http://www.w3.org/2001/XMLSchema#string"/>
  </owl:DatatypeProperty>
  <owl:DatatypeProperty rdf:about="http://example.org/onto/prop/google_chronicle_data_access_scope_asset_namespace">
    <rdfs:label>asset_namespace</rdfs:label>
    <rdfs:comment>The asset namespace configured in the forwarder
of the customer's events.</rdfs:comment>
    <rdfs:domain rdf:resource="http://example.org/onto/class/google_chronicle_data_access_scope"/>
    <rdfs:range rdf:resource="http://www.w3.org/2001/XMLSchema#string"/>
  </owl:DatatypeProperty>
  <owl:DatatypeProperty rdf:about="http://example.org/onto/prop/google_chronicle_data_access_scope_data_access_label">
    <rdfs:label>data_access_label</rdfs:label>
    <rdfs:comment>The name of the data access label.</rdfs:comment>
    <rdfs:domain rdf:resource="http://example.org/onto/class/google_chronicle_data_access_scope"/>
    <rdfs:range rdf:resource="http://www.w3.org/2001/XMLSchema#string"/>
  </owl:DatatypeProperty>
  <owl:DatatypeProperty rdf:about="http://example.org/onto/prop/google_chronicle_data_access_scope_display_name">
    <rdfs:label>display_name</rdfs:label>
    <rdfs:comment>Output only. The display name of the label.
Data access label and log types's name
will match the display name of the resource.
The asset namespace will match the namespace itself.
The ingestion key value pair will match the key of the tuple.</rdfs:comment>
    <rdfs:domain rdf:resource="http://example.org/onto/class/google_chronicle_data_access_scope"/>
    <rdfs:range rdf:resource="http://www.w3.org/2001/XMLSchema#string"/>
  </owl:DatatypeProperty>
  <owl:DatatypeProperty rdf:about="http://example.org/onto/prop/google_chronicle_data_access_scope_log_type">
    <rdfs:label>log_type</rdfs:label>
    <rdfs:comment>The name of the log type.</rdfs:comment>
    <rdfs:domain rdf:resource="http://example.org/onto/class/google_chronicle_data_access_scope"/>
    <rdfs:range rdf:resource="http://www.w3.org/2001/XMLSchema#string"/>
  </owl:DatatypeProperty>
  <owl:DatatypeProperty rdf:about="http://example.org/onto/prop/google_chronicle_data_access_scope_ingestion_label_key">
    <rdfs:label>ingestion_label_key</rdfs:label>
    <rdfs:comment>Required. The key of the ingestion label. Always required.</rdfs:comment>
    <rdfs:domain rdf:resource="http://example.org/onto/class/google_chronicle_data_access_scope"/>
    <rdfs:range rdf:resource="http://www.w3.org/2001/XMLSchema#string"/>
  </owl:DatatypeProperty>
  <owl:DatatypeProperty rdf:about="http://example.org/onto/prop/google_chronicle_data_access_scope_ingestion_label_value">
    <rdfs:label>ingestion_label_value</rdfs:label>
    <rdfs:comment>Optional. The value of the ingestion label. Optional. An object
with no provided value and some key provided would match
against the given key and ANY value.</rdfs:comment>
    <rdfs:domain rdf:resource="http://example.org/onto/class/google_chronicle_data_access_scope"/>
    <rdfs:range rdf:resource="http://www.w3.org/2001/XMLSchema#string"/>
  </owl:DatatypeProperty>
  <owl:DatatypeProperty rdf:about="http://example.org/onto/prop/google_chronicle_data_access_scope_create">
    <rdfs:label>create</rdfs:label>
    <rdfs:domain rdf:resource="http://example.org/onto/class/google_chronicle_data_access_scope"/>
    <rdfs:range rdf:resource="http://www.w3.org/2001/XMLSchema#string"/>
  </owl:DatatypeProperty>
  <owl:DatatypeProperty rdf:about="http://example.org/onto/prop/google_chronicle_data_access_scope_delete">
    <rdfs:label>delete</rdfs:label>
    <rdfs:domain rdf:resource="http://example.org/onto/class/google_chronicle_data_access_scope"/>
    <rdfs:range rdf:resource="http://www.w3.org/2001/XMLSchema#string"/>
  </owl:DatatypeProperty>
  <owl:DatatypeProperty rdf:about="http://example.org/onto/prop/google_chronicle_data_access_scope_update">
    <rdfs:label>update</rdfs:label>
    <rdfs:domain rdf:resource="http://example.org/onto/class/google_chronicle_data_access_scope"/>
    <rdfs:range rdf:resource="http://www.w3.org/2001/XMLSchema#string"/>
  </owl:DatatypeProperty>
</rdf:RDF>
