<?xml version="1.0" encoding="UTF-8"?>
<rdf:RDF
  xmlns:rdf="http://www.w3.org/1999/02/22-rdf-syntax-ns#"
  xmlns:rdfs="http://www.w3.org/2000/01/rdf-schema#"
  xmlns:owl="http://www.w3.org/2002/07/owl#"
  xmlns:xsd="http://www.w3.org/2001/XMLSchema#"
  xml:base="http://example.org/onto/">
  <owl:Class rdf:about="http://example.org/onto/class/google_sql_user">
    <rdfs:label>google_sql_user</rdfs:label>
    <rdfs:comment>#
#     ***     AUTO GENERATED CODE    ***    Type: Handwritten     ***
#
# ----------------------------------------------------------------------------
#
#     This code is generated by Magic Modules using the following:
#
#     Source file: https://github.com/GoogleCloudPlatform/magic-modules/tree/main/mmv1/third_party/terraform/website/docs/r/sql_user.html.markdown
#
#     DO NOT EDIT this file directly. Any changes made to this file will be
#     overwritten during the next generation cycle.
#
# ----------------------------------------------------------------------------
subcategory: "Cloud SQL"
description: |-
  Creates a new SQL user in Google Cloud SQL.
---</rdfs:comment>
  </owl:Class>
  <owl:DatatypeProperty rdf:about="http://example.org/onto/prop/google_sql_user_deletion_policy">
    <rdfs:label>deletion_policy</rdfs:label>
    <rdfs:comment>The deletion policy for the user. Setting ABANDON allows the resource
				to be abandoned rather than deleted. This is useful for Postgres, where users cannot be deleted from the API if they
				have been granted SQL roles. Possible values are: "ABANDON".</rdfs:comment>
    <rdfs:domain rdf:resource="http://example.org/onto/class/google_sql_user"/>
    <rdfs:range rdf:resource="http://www.w3.org/2001/XMLSchema#string"/>
  </owl:DatatypeProperty>
  <owl:DatatypeProperty rdf:about="http://example.org/onto/prop/google_sql_user_host">
    <rdfs:label>host</rdfs:label>
    <rdfs:comment>The host the user can connect from. This is only supported for MySQL instances. Don't set this field for PostgreSQL instances. Can be an IP address. Changing this forces a new resource to be created.</rdfs:comment>
    <rdfs:domain rdf:resource="http://example.org/onto/class/google_sql_user"/>
    <rdfs:range rdf:resource="http://www.w3.org/2001/XMLSchema#string"/>
  </owl:DatatypeProperty>
  <owl:DatatypeProperty rdf:about="http://example.org/onto/prop/google_sql_user_id">
    <rdfs:label>id</rdfs:label>
    <rdfs:domain rdf:resource="http://example.org/onto/class/google_sql_user"/>
    <rdfs:range rdf:resource="http://www.w3.org/2001/XMLSchema#string"/>
  </owl:DatatypeProperty>
  <owl:DatatypeProperty rdf:about="http://example.org/onto/prop/google_sql_user_instance">
    <rdfs:label>instance</rdfs:label>
    <rdfs:comment>The name of the Cloud SQL instance. Changing this forces a new resource to be created.</rdfs:comment>
    <rdfs:domain rdf:resource="http://example.org/onto/class/google_sql_user"/>
    <rdfs:range rdf:resource="http://www.w3.org/2001/XMLSchema#string"/>
  </owl:DatatypeProperty>
  <owl:DatatypeProperty rdf:about="http://example.org/onto/prop/google_sql_user_name">
    <rdfs:label>name</rdfs:label>
    <rdfs:comment>The name of the user. Changing this forces a new resource to be created.</rdfs:comment>
    <rdfs:domain rdf:resource="http://example.org/onto/class/google_sql_user"/>
    <rdfs:range rdf:resource="http://www.w3.org/2001/XMLSchema#string"/>
  </owl:DatatypeProperty>
  <owl:DatatypeProperty rdf:about="http://example.org/onto/prop/google_sql_user_password">
    <rdfs:label>password</rdfs:label>
    <rdfs:comment>The password for the user. Can be updated. For Postgres instances this is a Required field, unless type is set to
				either CLOUD_IAM_USER or CLOUD_IAM_SERVICE_ACCOUNT.</rdfs:comment>
    <rdfs:domain rdf:resource="http://example.org/onto/class/google_sql_user"/>
    <rdfs:range rdf:resource="http://www.w3.org/2001/XMLSchema#string"/>
  </owl:DatatypeProperty>
  <owl:DatatypeProperty rdf:about="http://example.org/onto/prop/google_sql_user_password_wo">
    <rdfs:label>password_wo</rdfs:label>
    <rdfs:comment>The password for the user. Can be updated. For Postgres instances this is a Required field, unless type is set to
				either CLOUD_IAM_USER or CLOUD_IAM_SERVICE_ACCOUNT.</rdfs:comment>
    <rdfs:domain rdf:resource="http://example.org/onto/class/google_sql_user"/>
    <rdfs:range rdf:resource="http://www.w3.org/2001/XMLSchema#string"/>
  </owl:DatatypeProperty>
  <owl:DatatypeProperty rdf:about="http://example.org/onto/prop/google_sql_user_password_wo_version">
    <rdfs:label>password_wo_version</rdfs:label>
    <rdfs:comment>The version of the password_wo.</rdfs:comment>
    <rdfs:domain rdf:resource="http://example.org/onto/class/google_sql_user"/>
    <rdfs:range rdf:resource="http://www.w3.org/2001/XMLSchema#string"/>
  </owl:DatatypeProperty>
  <owl:DatatypeProperty rdf:about="http://example.org/onto/prop/google_sql_user_project">
    <rdfs:label>project</rdfs:label>
    <rdfs:comment>The ID of the project in which the resource belongs. If it is not provided, the provider project is used.</rdfs:comment>
    <rdfs:domain rdf:resource="http://example.org/onto/class/google_sql_user"/>
    <rdfs:range rdf:resource="http://www.w3.org/2001/XMLSchema#string"/>
  </owl:DatatypeProperty>
  <owl:DatatypeProperty rdf:about="http://example.org/onto/prop/google_sql_user_sql_server_user_details">
    <rdfs:label>sql_server_user_details</rdfs:label>
    <rdfs:domain rdf:resource="http://example.org/onto/class/google_sql_user"/>
    <rdfs:range rdf:resource="http://www.w3.org/2001/XMLSchema#string"/>
  </owl:DatatypeProperty>
  <owl:DatatypeProperty rdf:about="http://example.org/onto/prop/google_sql_user_type">
    <rdfs:label>type</rdfs:label>
    <rdfs:comment>The user type. It determines the method to authenticate the user during login.
				The default is the database's built-in user type.</rdfs:comment>
    <rdfs:domain rdf:resource="http://example.org/onto/class/google_sql_user"/>
    <rdfs:range rdf:resource="http://www.w3.org/2001/XMLSchema#string"/>
  </owl:DatatypeProperty>
  <owl:DatatypeProperty rdf:about="http://example.org/onto/prop/google_sql_user_allowed_failed_attempts">
    <rdfs:label>allowed_failed_attempts</rdfs:label>
    <rdfs:comment>Number of failed attempts allowed before the user get locked.</rdfs:comment>
    <rdfs:domain rdf:resource="http://example.org/onto/class/google_sql_user"/>
    <rdfs:range rdf:resource="http://www.w3.org/2001/XMLSchema#string"/>
  </owl:DatatypeProperty>
  <owl:DatatypeProperty rdf:about="http://example.org/onto/prop/google_sql_user_enable_failed_attempts_check">
    <rdfs:label>enable_failed_attempts_check</rdfs:label>
    <rdfs:comment>If true, the check that will lock user after too many failed login attempts will be enabled.</rdfs:comment>
    <rdfs:domain rdf:resource="http://example.org/onto/class/google_sql_user"/>
    <rdfs:range rdf:resource="http://www.w3.org/2001/XMLSchema#string"/>
  </owl:DatatypeProperty>
  <owl:DatatypeProperty rdf:about="http://example.org/onto/prop/google_sql_user_enable_password_verification">
    <rdfs:label>enable_password_verification</rdfs:label>
    <rdfs:comment>If true, the user must specify the current password before changing the password. This flag is supported only for MySQL.</rdfs:comment>
    <rdfs:domain rdf:resource="http://example.org/onto/class/google_sql_user"/>
    <rdfs:range rdf:resource="http://www.w3.org/2001/XMLSchema#string"/>
  </owl:DatatypeProperty>
  <owl:DatatypeProperty rdf:about="http://example.org/onto/prop/google_sql_user_password_expiration_duration">
    <rdfs:label>password_expiration_duration</rdfs:label>
    <rdfs:comment>Password expiration duration with one week grace period.</rdfs:comment>
    <rdfs:domain rdf:resource="http://example.org/onto/class/google_sql_user"/>
    <rdfs:range rdf:resource="http://www.w3.org/2001/XMLSchema#string"/>
  </owl:DatatypeProperty>
  <owl:DatatypeProperty rdf:about="http://example.org/onto/prop/google_sql_user_status">
    <rdfs:label>status</rdfs:label>
    <rdfs:domain rdf:resource="http://example.org/onto/class/google_sql_user"/>
    <rdfs:range rdf:resource="http://www.w3.org/2001/XMLSchema#string"/>
  </owl:DatatypeProperty>
  <owl:DatatypeProperty rdf:about="http://example.org/onto/prop/google_sql_user_create">
    <rdfs:label>create</rdfs:label>
    <rdfs:domain rdf:resource="http://example.org/onto/class/google_sql_user"/>
    <rdfs:range rdf:resource="http://www.w3.org/2001/XMLSchema#string"/>
  </owl:DatatypeProperty>
  <owl:DatatypeProperty rdf:about="http://example.org/onto/prop/google_sql_user_delete">
    <rdfs:label>delete</rdfs:label>
    <rdfs:domain rdf:resource="http://example.org/onto/class/google_sql_user"/>
    <rdfs:range rdf:resource="http://www.w3.org/2001/XMLSchema#string"/>
  </owl:DatatypeProperty>
  <owl:DatatypeProperty rdf:about="http://example.org/onto/prop/google_sql_user_update">
    <rdfs:label>update</rdfs:label>
    <rdfs:domain rdf:resource="http://example.org/onto/class/google_sql_user"/>
    <rdfs:range rdf:resource="http://www.w3.org/2001/XMLSchema#string"/>
  </owl:DatatypeProperty>
</rdf:RDF>
