<?xml version="1.0" encoding="UTF-8"?>
<rdf:RDF
  xmlns:rdf="http://www.w3.org/1999/02/22-rdf-syntax-ns#"
  xmlns:rdfs="http://www.w3.org/2000/01/rdf-schema#"
  xmlns:owl="http://www.w3.org/2002/07/owl#"
  xmlns:xsd="http://www.w3.org/2001/XMLSchema#"
  xml:base="http://example.org/onto/">
  <owl:Class rdf:about="http://example.org/onto/class/google_eventarc_trigger">
    <rdfs:label>google_eventarc_trigger</rdfs:label>
    <rdfs:comment>#
#     ***     AUTO GENERATED CODE    ***    Type: MMv1     ***
#
# ----------------------------------------------------------------------------
#
#     This code is generated by Magic Modules using the following:
#
#     Configuration: https:#github.com/GoogleCloudPlatform/magic-modules/tree/main/mmv1/products/eventarc/Trigger.yaml
#     Template:      https:#github.com/GoogleCloudPlatform/magic-modules/tree/main/mmv1/templates/terraform/resource.html.markdown.tmpl
#
#     DO NOT EDIT this file directly. Any changes made to this file will be
#     overwritten during the next generation cycle.
#
# ----------------------------------------------------------------------------
subcategory: "Eventarc"
description: |-
  The Eventarc Trigger resource
---</rdfs:comment>
  </owl:Class>
  <owl:DatatypeProperty rdf:about="http://example.org/onto/prop/google_eventarc_trigger_channel">
    <rdfs:label>channel</rdfs:label>
    <rdfs:comment>Optional. The name of the channel associated with the trigger in 'projects/{project}/locations/{location}/channels/{channel}' format. You must provide a channel to receive events from Eventarc SaaS partners.</rdfs:comment>
    <rdfs:domain rdf:resource="http://example.org/onto/class/google_eventarc_trigger"/>
    <rdfs:range rdf:resource="http://www.w3.org/2001/XMLSchema#string"/>
  </owl:DatatypeProperty>
  <owl:DatatypeProperty rdf:about="http://example.org/onto/prop/google_eventarc_trigger_conditions">
    <rdfs:label>conditions</rdfs:label>
    <rdfs:comment>Output only. The reason(s) why a trigger is in FAILED state.</rdfs:comment>
    <rdfs:domain rdf:resource="http://example.org/onto/class/google_eventarc_trigger"/>
    <rdfs:range rdf:resource="http://www.w3.org/2001/XMLSchema#string"/>
  </owl:DatatypeProperty>
  <owl:DatatypeProperty rdf:about="http://example.org/onto/prop/google_eventarc_trigger_create_time">
    <rdfs:label>create_time</rdfs:label>
    <rdfs:comment>Output only. The creation time.</rdfs:comment>
    <rdfs:domain rdf:resource="http://example.org/onto/class/google_eventarc_trigger"/>
    <rdfs:range rdf:resource="http://www.w3.org/2001/XMLSchema#string"/>
  </owl:DatatypeProperty>
  <owl:DatatypeProperty rdf:about="http://example.org/onto/prop/google_eventarc_trigger_effective_labels">
    <rdfs:label>effective_labels</rdfs:label>
    <rdfs:comment>All of labels (key/value pairs) present on the resource in GCP, including the labels configured through Terraform, other clients and services.</rdfs:comment>
    <rdfs:domain rdf:resource="http://example.org/onto/class/google_eventarc_trigger"/>
    <rdfs:range rdf:resource="http://www.w3.org/2001/XMLSchema#string"/>
  </owl:DatatypeProperty>
  <owl:DatatypeProperty rdf:about="http://example.org/onto/prop/google_eventarc_trigger_etag">
    <rdfs:label>etag</rdfs:label>
    <rdfs:comment>Output only. This checksum is computed by the server based on the value of other fields, and may be sent only on create requests to ensure the client has an up-to-date value before proceeding.</rdfs:comment>
    <rdfs:domain rdf:resource="http://example.org/onto/class/google_eventarc_trigger"/>
    <rdfs:range rdf:resource="http://www.w3.org/2001/XMLSchema#string"/>
  </owl:DatatypeProperty>
  <owl:DatatypeProperty rdf:about="http://example.org/onto/prop/google_eventarc_trigger_event_data_content_type">
    <rdfs:label>event_data_content_type</rdfs:label>
    <rdfs:comment>Optional. EventDataContentType specifies the type of payload in MIME format that is expected from the CloudEvent data field. This is set to 'application/json' if the value is not defined.</rdfs:comment>
    <rdfs:domain rdf:resource="http://example.org/onto/class/google_eventarc_trigger"/>
    <rdfs:range rdf:resource="http://www.w3.org/2001/XMLSchema#string"/>
  </owl:DatatypeProperty>
  <owl:DatatypeProperty rdf:about="http://example.org/onto/prop/google_eventarc_trigger_id">
    <rdfs:label>id</rdfs:label>
    <rdfs:domain rdf:resource="http://example.org/onto/class/google_eventarc_trigger"/>
    <rdfs:range rdf:resource="http://www.w3.org/2001/XMLSchema#string"/>
  </owl:DatatypeProperty>
  <owl:DatatypeProperty rdf:about="http://example.org/onto/prop/google_eventarc_trigger_labels">
    <rdfs:label>labels</rdfs:label>
    <rdfs:comment>Optional. User labels attached to the triggers that can be used to group resources.

**Note**: This field is non-authoritative, and will only manage the labels present in your configuration.
Please refer to the field 'effective_labels' for all of the labels present on the resource.</rdfs:comment>
    <rdfs:domain rdf:resource="http://example.org/onto/class/google_eventarc_trigger"/>
    <rdfs:range rdf:resource="http://www.w3.org/2001/XMLSchema#string"/>
  </owl:DatatypeProperty>
  <owl:DatatypeProperty rdf:about="http://example.org/onto/prop/google_eventarc_trigger_location">
    <rdfs:label>location</rdfs:label>
    <rdfs:comment>The location for the resource</rdfs:comment>
    <rdfs:domain rdf:resource="http://example.org/onto/class/google_eventarc_trigger"/>
    <rdfs:range rdf:resource="http://www.w3.org/2001/XMLSchema#string"/>
  </owl:DatatypeProperty>
  <owl:DatatypeProperty rdf:about="http://example.org/onto/prop/google_eventarc_trigger_name">
    <rdfs:label>name</rdfs:label>
    <rdfs:comment>Required. The resource name of the trigger. Must be unique within the location on the project.</rdfs:comment>
    <rdfs:domain rdf:resource="http://example.org/onto/class/google_eventarc_trigger"/>
    <rdfs:range rdf:resource="http://www.w3.org/2001/XMLSchema#string"/>
  </owl:DatatypeProperty>
  <owl:DatatypeProperty rdf:about="http://example.org/onto/prop/google_eventarc_trigger_project">
    <rdfs:label>project</rdfs:label>
    <rdfs:domain rdf:resource="http://example.org/onto/class/google_eventarc_trigger"/>
    <rdfs:range rdf:resource="http://www.w3.org/2001/XMLSchema#string"/>
  </owl:DatatypeProperty>
  <owl:DatatypeProperty rdf:about="http://example.org/onto/prop/google_eventarc_trigger_service_account">
    <rdfs:label>service_account</rdfs:label>
    <rdfs:comment>Optional. The IAM service account email associated with the trigger. The service account represents the identity of the trigger. The principal who calls this API must have 'iam.serviceAccounts.actAs' permission in the service account. See https://cloud.google.com/iam/docs/understanding-service-accounts#sa_common for more information. For Cloud Run destinations, this service account is used to generate identity tokens when invoking the service. See https://cloud.google.com/run/docs/triggering/pubsub-push#create-service-account for information on how to invoke authenticated Cloud Run services. In order to create Audit Log triggers, the service account should also have 'roles/eventarc.eventReceiver' IAM role.</rdfs:comment>
    <rdfs:domain rdf:resource="http://example.org/onto/class/google_eventarc_trigger"/>
    <rdfs:range rdf:resource="http://www.w3.org/2001/XMLSchema#string"/>
  </owl:DatatypeProperty>
  <owl:DatatypeProperty rdf:about="http://example.org/onto/prop/google_eventarc_trigger_terraform_labels">
    <rdfs:label>terraform_labels</rdfs:label>
    <rdfs:comment>The combination of labels configured directly on the resource
 and default labels configured on the provider.</rdfs:comment>
    <rdfs:domain rdf:resource="http://example.org/onto/class/google_eventarc_trigger"/>
    <rdfs:range rdf:resource="http://www.w3.org/2001/XMLSchema#string"/>
  </owl:DatatypeProperty>
  <owl:DatatypeProperty rdf:about="http://example.org/onto/prop/google_eventarc_trigger_uid">
    <rdfs:label>uid</rdfs:label>
    <rdfs:comment>Output only. Server assigned unique identifier for the trigger. The value is a UUID4 string and guaranteed to remain unchanged until the resource is deleted.</rdfs:comment>
    <rdfs:domain rdf:resource="http://example.org/onto/class/google_eventarc_trigger"/>
    <rdfs:range rdf:resource="http://www.w3.org/2001/XMLSchema#string"/>
  </owl:DatatypeProperty>
  <owl:DatatypeProperty rdf:about="http://example.org/onto/prop/google_eventarc_trigger_update_time">
    <rdfs:label>update_time</rdfs:label>
    <rdfs:comment>Output only. The last-modified time.</rdfs:comment>
    <rdfs:domain rdf:resource="http://example.org/onto/class/google_eventarc_trigger"/>
    <rdfs:range rdf:resource="http://www.w3.org/2001/XMLSchema#string"/>
  </owl:DatatypeProperty>
  <owl:DatatypeProperty rdf:about="http://example.org/onto/prop/google_eventarc_trigger_cloud_function">
    <rdfs:label>cloud_function</rdfs:label>
    <rdfs:comment>The Cloud Function resource name. Only Cloud Functions V2 is supported. Format projects/{project}/locations/{location}/functions/{function} This is a read-only field. [WARNING] Creating Cloud Functions V2 triggers is only supported via the Cloud Functions product. An error will be returned if the user sets this value.</rdfs:comment>
    <rdfs:domain rdf:resource="http://example.org/onto/class/google_eventarc_trigger"/>
    <rdfs:range rdf:resource="http://www.w3.org/2001/XMLSchema#string"/>
  </owl:DatatypeProperty>
  <owl:DatatypeProperty rdf:about="http://example.org/onto/prop/google_eventarc_trigger_workflow">
    <rdfs:label>workflow</rdfs:label>
    <rdfs:comment>The resource name of the Workflow whose Executions are triggered by the events. The Workflow resource should be deployed in the same project as the trigger. Format: 'projects/{project}/locations/{location}/workflows/{workflow}'</rdfs:comment>
    <rdfs:domain rdf:resource="http://example.org/onto/class/google_eventarc_trigger"/>
    <rdfs:range rdf:resource="http://www.w3.org/2001/XMLSchema#string"/>
  </owl:DatatypeProperty>
  <owl:DatatypeProperty rdf:about="http://example.org/onto/prop/google_eventarc_trigger_path">
    <rdfs:label>path</rdfs:label>
    <rdfs:comment>Optional. The relative path on the Cloud Run service the events should be sent to. The value must conform to the definition of URI path segment (section 3.3 of RFC2396). Examples: "/route", "route", "route/subroute".</rdfs:comment>
    <rdfs:domain rdf:resource="http://example.org/onto/class/google_eventarc_trigger"/>
    <rdfs:range rdf:resource="http://www.w3.org/2001/XMLSchema#string"/>
  </owl:DatatypeProperty>
  <owl:DatatypeProperty rdf:about="http://example.org/onto/prop/google_eventarc_trigger_region">
    <rdfs:label>region</rdfs:label>
    <rdfs:comment>Required. The region the Cloud Run service is deployed in.</rdfs:comment>
    <rdfs:domain rdf:resource="http://example.org/onto/class/google_eventarc_trigger"/>
    <rdfs:range rdf:resource="http://www.w3.org/2001/XMLSchema#string"/>
  </owl:DatatypeProperty>
  <owl:DatatypeProperty rdf:about="http://example.org/onto/prop/google_eventarc_trigger_service">
    <rdfs:label>service</rdfs:label>
    <rdfs:comment>Required. The name of the Cloud Run service being addressed. See https://cloud.google.com/run/docs/reference/rest/v1/namespaces.services. Only services located in the same project of the trigger object can be addressed.</rdfs:comment>
    <rdfs:domain rdf:resource="http://example.org/onto/class/google_eventarc_trigger"/>
    <rdfs:range rdf:resource="http://www.w3.org/2001/XMLSchema#string"/>
  </owl:DatatypeProperty>
  <owl:DatatypeProperty rdf:about="http://example.org/onto/prop/google_eventarc_trigger_cluster">
    <rdfs:label>cluster</rdfs:label>
    <rdfs:comment>Required. The name of the cluster the GKE service is running in. The cluster must be running in the same project as the trigger being created.</rdfs:comment>
    <rdfs:domain rdf:resource="http://example.org/onto/class/google_eventarc_trigger"/>
    <rdfs:range rdf:resource="http://www.w3.org/2001/XMLSchema#string"/>
  </owl:DatatypeProperty>
  <owl:DatatypeProperty rdf:about="http://example.org/onto/prop/google_eventarc_trigger_location">
    <rdfs:label>location</rdfs:label>
    <rdfs:comment>Required. The name of the Google Compute Engine in which the cluster resides, which can either be compute zone (for example, us-central1-a) for the zonal clusters or region (for example, us-central1) for regional clusters.</rdfs:comment>
    <rdfs:domain rdf:resource="http://example.org/onto/class/google_eventarc_trigger"/>
    <rdfs:range rdf:resource="http://www.w3.org/2001/XMLSchema#string"/>
  </owl:DatatypeProperty>
  <owl:DatatypeProperty rdf:about="http://example.org/onto/prop/google_eventarc_trigger_namespace">
    <rdfs:label>namespace</rdfs:label>
    <rdfs:comment>Required. The namespace the GKE service is running in.</rdfs:comment>
    <rdfs:domain rdf:resource="http://example.org/onto/class/google_eventarc_trigger"/>
    <rdfs:range rdf:resource="http://www.w3.org/2001/XMLSchema#string"/>
  </owl:DatatypeProperty>
  <owl:DatatypeProperty rdf:about="http://example.org/onto/prop/google_eventarc_trigger_path">
    <rdfs:label>path</rdfs:label>
    <rdfs:comment>Optional. The relative path on the GKE service the events should be sent to. The value must conform to the definition of a URI path segment (section 3.3 of RFC2396). Examples: "/route", "route", "route/subroute".</rdfs:comment>
    <rdfs:domain rdf:resource="http://example.org/onto/class/google_eventarc_trigger"/>
    <rdfs:range rdf:resource="http://www.w3.org/2001/XMLSchema#string"/>
  </owl:DatatypeProperty>
  <owl:DatatypeProperty rdf:about="http://example.org/onto/prop/google_eventarc_trigger_service">
    <rdfs:label>service</rdfs:label>
    <rdfs:comment>Required. Name of the GKE service.</rdfs:comment>
    <rdfs:domain rdf:resource="http://example.org/onto/class/google_eventarc_trigger"/>
    <rdfs:range rdf:resource="http://www.w3.org/2001/XMLSchema#string"/>
  </owl:DatatypeProperty>
  <owl:DatatypeProperty rdf:about="http://example.org/onto/prop/google_eventarc_trigger_uri">
    <rdfs:label>uri</rdfs:label>
    <rdfs:comment>Required. The URI of the HTTP enpdoint. The value must be a RFC2396 URI string. Examples: 'http://10.10.10.8:80/route', 'http://svc.us-central1.p.local:8080/'. Only HTTP and HTTPS protocols are supported. The host can be either a static IP addressable from the VPC specified by the network config, or an internal DNS hostname of the service resolvable via Cloud DNS.</rdfs:comment>
    <rdfs:domain rdf:resource="http://example.org/onto/class/google_eventarc_trigger"/>
    <rdfs:range rdf:resource="http://www.w3.org/2001/XMLSchema#string"/>
  </owl:DatatypeProperty>
  <owl:DatatypeProperty rdf:about="http://example.org/onto/prop/google_eventarc_trigger_network_attachment">
    <rdfs:label>network_attachment</rdfs:label>
    <rdfs:comment>Required. Name of the NetworkAttachment that allows access to the destination VPC. Format: 'projects/{PROJECT_ID}/regions/{REGION}/networkAttachments/{NETWORK_ATTACHMENT_NAME}'</rdfs:comment>
    <rdfs:domain rdf:resource="http://example.org/onto/class/google_eventarc_trigger"/>
    <rdfs:range rdf:resource="http://www.w3.org/2001/XMLSchema#string"/>
  </owl:DatatypeProperty>
  <owl:DatatypeProperty rdf:about="http://example.org/onto/prop/google_eventarc_trigger_attribute">
    <rdfs:label>attribute</rdfs:label>
    <rdfs:comment>Required. The name of a CloudEvents attribute. Currently, only a subset of attributes are supported for filtering. All triggers MUST provide a filter for the 'type' attribute.</rdfs:comment>
    <rdfs:domain rdf:resource="http://example.org/onto/class/google_eventarc_trigger"/>
    <rdfs:range rdf:resource="http://www.w3.org/2001/XMLSchema#string"/>
  </owl:DatatypeProperty>
  <owl:DatatypeProperty rdf:about="http://example.org/onto/prop/google_eventarc_trigger_operator">
    <rdfs:label>operator</rdfs:label>
    <rdfs:comment>Optional. The operator used for matching the events with the value of the filter. If not specified, only events that have an exact key-value pair specified in the filter are matched. The only allowed value is 'match-path-pattern'.</rdfs:comment>
    <rdfs:domain rdf:resource="http://example.org/onto/class/google_eventarc_trigger"/>
    <rdfs:range rdf:resource="http://www.w3.org/2001/XMLSchema#string"/>
  </owl:DatatypeProperty>
  <owl:DatatypeProperty rdf:about="http://example.org/onto/prop/google_eventarc_trigger_value">
    <rdfs:label>value</rdfs:label>
    <rdfs:comment>Required. The value for the attribute. See https://cloud.google.com/eventarc/docs/creating-triggers#trigger-gcloud for available values.</rdfs:comment>
    <rdfs:domain rdf:resource="http://example.org/onto/class/google_eventarc_trigger"/>
    <rdfs:range rdf:resource="http://www.w3.org/2001/XMLSchema#string"/>
  </owl:DatatypeProperty>
  <owl:DatatypeProperty rdf:about="http://example.org/onto/prop/google_eventarc_trigger_create">
    <rdfs:label>create</rdfs:label>
    <rdfs:domain rdf:resource="http://example.org/onto/class/google_eventarc_trigger"/>
    <rdfs:range rdf:resource="http://www.w3.org/2001/XMLSchema#string"/>
  </owl:DatatypeProperty>
  <owl:DatatypeProperty rdf:about="http://example.org/onto/prop/google_eventarc_trigger_delete">
    <rdfs:label>delete</rdfs:label>
    <rdfs:domain rdf:resource="http://example.org/onto/class/google_eventarc_trigger"/>
    <rdfs:range rdf:resource="http://www.w3.org/2001/XMLSchema#string"/>
  </owl:DatatypeProperty>
  <owl:DatatypeProperty rdf:about="http://example.org/onto/prop/google_eventarc_trigger_update">
    <rdfs:label>update</rdfs:label>
    <rdfs:domain rdf:resource="http://example.org/onto/class/google_eventarc_trigger"/>
    <rdfs:range rdf:resource="http://www.w3.org/2001/XMLSchema#string"/>
  </owl:DatatypeProperty>
  <owl:DatatypeProperty rdf:about="http://example.org/onto/prop/google_eventarc_trigger_subscription">
    <rdfs:label>subscription</rdfs:label>
    <rdfs:comment>Output only. The name of the Pub/Sub subscription created and managed by Eventarc system as a transport for the event delivery. Format: 'projects/{PROJECT_ID}/subscriptions/{SUBSCRIPTION_NAME}'.</rdfs:comment>
    <rdfs:domain rdf:resource="http://example.org/onto/class/google_eventarc_trigger"/>
    <rdfs:range rdf:resource="http://www.w3.org/2001/XMLSchema#string"/>
  </owl:DatatypeProperty>
  <owl:DatatypeProperty rdf:about="http://example.org/onto/prop/google_eventarc_trigger_topic">
    <rdfs:label>topic</rdfs:label>
    <rdfs:comment>Optional. The name of the Pub/Sub topic created and managed by Eventarc system as a transport for the event delivery. Format: 'projects/{PROJECT_ID}/topics/{TOPIC_NAME}. You may set an existing topic for triggers of the type google.cloud.pubsub.topic.v1.messagePublished' only. The topic you provide here will not be deleted by Eventarc at trigger deletion.</rdfs:comment>
    <rdfs:domain rdf:resource="http://example.org/onto/class/google_eventarc_trigger"/>
    <rdfs:range rdf:resource="http://www.w3.org/2001/XMLSchema#string"/>
  </owl:DatatypeProperty>
</rdf:RDF>
