<?xml version="1.0" encoding="UTF-8"?>
<rdf:RDF
  xmlns:rdf="http://www.w3.org/1999/02/22-rdf-syntax-ns#"
  xmlns:rdfs="http://www.w3.org/2000/01/rdf-schema#"
  xmlns:owl="http://www.w3.org/2002/07/owl#"
  xmlns:xsd="http://www.w3.org/2001/XMLSchema#"
  xml:base="http://example.org/onto/">
  <owl:Class rdf:about="http://example.org/onto/class/google_clouddeploy_deploy_policy">
    <rdfs:label>google_clouddeploy_deploy_policy</rdfs:label>
    <rdfs:comment>#
#     ***     AUTO GENERATED CODE    ***    Type: MMv1     ***
#
# ----------------------------------------------------------------------------
#
#     This code is generated by Magic Modules using the following:
#
#     Configuration: https:#github.com/GoogleCloudPlatform/magic-modules/tree/main/mmv1/products/clouddeploy/DeployPolicy.yaml
#     Template:      https:#github.com/GoogleCloudPlatform/magic-modules/tree/main/mmv1/templates/terraform/resource.html.markdown.tmpl
#
#     DO NOT EDIT this file directly. Any changes made to this file will be
#     overwritten during the next generation cycle.
#
# ----------------------------------------------------------------------------
subcategory: "Cloud Deploy"
description: |-
  A `DeployPolicy` inhibits manual or DeployPolicy-driven actions within a Delivery Pipeline or Target.
---</rdfs:comment>
  </owl:Class>
  <owl:DatatypeProperty rdf:about="http://example.org/onto/prop/google_clouddeploy_deploy_policy_annotations">
    <rdfs:label>annotations</rdfs:label>
    <rdfs:comment>User annotations. These attributes can only be set and used by the user, and not by Cloud Deploy. Annotations must meet the following constraints: * Annotations are key/value pairs. * Valid annotation keys have two segments: an optional prefix and name, separated by a slash ('/'). * The name segment is required and must be 63 characters or less, beginning and ending with an alphanumeric character ('[a-z0-9A-Z]') with dashes ('-'), underscores ('_'), dots ('.'), and alphanumerics between. * The prefix is optional. If specified, the prefix must be a DNS subdomain: a series of DNS labels separated by dots('.'), not longer than 253 characters in total, followed by a slash ('/'). See https://kubernetes.io/docs/concepts/overview/working-with-objects/annotations/#syntax-and-character-set for more details.

**Note**: This field is non-authoritative, and will only manage the annotations present in your configuration.
Please refer to the field 'effective_annotations' for all of the annotations present on the resource.</rdfs:comment>
    <rdfs:domain rdf:resource="http://example.org/onto/class/google_clouddeploy_deploy_policy"/>
    <rdfs:range rdf:resource="http://www.w3.org/2001/XMLSchema#string"/>
  </owl:DatatypeProperty>
  <owl:DatatypeProperty rdf:about="http://example.org/onto/prop/google_clouddeploy_deploy_policy_create_time">
    <rdfs:label>create_time</rdfs:label>
    <rdfs:comment>Output only. Time at which the DeployPolicy was created.</rdfs:comment>
    <rdfs:domain rdf:resource="http://example.org/onto/class/google_clouddeploy_deploy_policy"/>
    <rdfs:range rdf:resource="http://www.w3.org/2001/XMLSchema#string"/>
  </owl:DatatypeProperty>
  <owl:DatatypeProperty rdf:about="http://example.org/onto/prop/google_clouddeploy_deploy_policy_description">
    <rdfs:label>description</rdfs:label>
    <rdfs:comment>Description of the 'DeployPolicy'. Max length is 255 characters.</rdfs:comment>
    <rdfs:domain rdf:resource="http://example.org/onto/class/google_clouddeploy_deploy_policy"/>
    <rdfs:range rdf:resource="http://www.w3.org/2001/XMLSchema#string"/>
  </owl:DatatypeProperty>
  <owl:DatatypeProperty rdf:about="http://example.org/onto/prop/google_clouddeploy_deploy_policy_effective_annotations">
    <rdfs:label>effective_annotations</rdfs:label>
    <rdfs:comment>All of annotations (key/value pairs) present on the resource in GCP, including the annotations configured through Terraform, other clients and services.</rdfs:comment>
    <rdfs:domain rdf:resource="http://example.org/onto/class/google_clouddeploy_deploy_policy"/>
    <rdfs:range rdf:resource="http://www.w3.org/2001/XMLSchema#string"/>
  </owl:DatatypeProperty>
  <owl:DatatypeProperty rdf:about="http://example.org/onto/prop/google_clouddeploy_deploy_policy_effective_labels">
    <rdfs:label>effective_labels</rdfs:label>
    <rdfs:comment>All of labels (key/value pairs) present on the resource in GCP, including the labels configured through Terraform, other clients and services.</rdfs:comment>
    <rdfs:domain rdf:resource="http://example.org/onto/class/google_clouddeploy_deploy_policy"/>
    <rdfs:range rdf:resource="http://www.w3.org/2001/XMLSchema#string"/>
  </owl:DatatypeProperty>
  <owl:DatatypeProperty rdf:about="http://example.org/onto/prop/google_clouddeploy_deploy_policy_etag">
    <rdfs:label>etag</rdfs:label>
    <rdfs:comment>The weak etag of the 'DeployPolicy' resource. This checksum is computed by the server based on the value of other fields, and may be sent on update and delete requests to ensure the client has an up-to-date value before proceeding.</rdfs:comment>
    <rdfs:domain rdf:resource="http://example.org/onto/class/google_clouddeploy_deploy_policy"/>
    <rdfs:range rdf:resource="http://www.w3.org/2001/XMLSchema#string"/>
  </owl:DatatypeProperty>
  <owl:DatatypeProperty rdf:about="http://example.org/onto/prop/google_clouddeploy_deploy_policy_id">
    <rdfs:label>id</rdfs:label>
    <rdfs:domain rdf:resource="http://example.org/onto/class/google_clouddeploy_deploy_policy"/>
    <rdfs:range rdf:resource="http://www.w3.org/2001/XMLSchema#string"/>
  </owl:DatatypeProperty>
  <owl:DatatypeProperty rdf:about="http://example.org/onto/prop/google_clouddeploy_deploy_policy_labels">
    <rdfs:label>labels</rdfs:label>
    <rdfs:comment>Labels are attributes that can be set and used by both the user and by Cloud Deploy. Labels must meet the following constraints: * Keys and values can contain only lowercase letters, numeric characters, underscores, and dashes. * All characters must use UTF-8 encoding, and international characters are allowed. * Keys must start with a lowercase letter or international character. * Each resource is limited to a maximum of 64 labels. Both keys and values are additionally constrained to be <= 63 characters.

**Note**: This field is non-authoritative, and will only manage the labels present in your configuration.
Please refer to the field 'effective_labels' for all of the labels present on the resource.</rdfs:comment>
    <rdfs:domain rdf:resource="http://example.org/onto/class/google_clouddeploy_deploy_policy"/>
    <rdfs:range rdf:resource="http://www.w3.org/2001/XMLSchema#string"/>
  </owl:DatatypeProperty>
  <owl:DatatypeProperty rdf:about="http://example.org/onto/prop/google_clouddeploy_deploy_policy_location">
    <rdfs:label>location</rdfs:label>
    <rdfs:comment>The location for the resource</rdfs:comment>
    <rdfs:domain rdf:resource="http://example.org/onto/class/google_clouddeploy_deploy_policy"/>
    <rdfs:range rdf:resource="http://www.w3.org/2001/XMLSchema#string"/>
  </owl:DatatypeProperty>
  <owl:DatatypeProperty rdf:about="http://example.org/onto/prop/google_clouddeploy_deploy_policy_name">
    <rdfs:label>name</rdfs:label>
    <rdfs:comment>Name of the 'DeployPolicy'.</rdfs:comment>
    <rdfs:domain rdf:resource="http://example.org/onto/class/google_clouddeploy_deploy_policy"/>
    <rdfs:range rdf:resource="http://www.w3.org/2001/XMLSchema#string"/>
  </owl:DatatypeProperty>
  <owl:DatatypeProperty rdf:about="http://example.org/onto/prop/google_clouddeploy_deploy_policy_project">
    <rdfs:label>project</rdfs:label>
    <rdfs:domain rdf:resource="http://example.org/onto/class/google_clouddeploy_deploy_policy"/>
    <rdfs:range rdf:resource="http://www.w3.org/2001/XMLSchema#string"/>
  </owl:DatatypeProperty>
  <owl:DatatypeProperty rdf:about="http://example.org/onto/prop/google_clouddeploy_deploy_policy_suspended">
    <rdfs:label>suspended</rdfs:label>
    <rdfs:comment>When suspended, the policy will not prevent actions from occurring, even if the action violates the policy.</rdfs:comment>
    <rdfs:domain rdf:resource="http://example.org/onto/class/google_clouddeploy_deploy_policy"/>
    <rdfs:range rdf:resource="http://www.w3.org/2001/XMLSchema#string"/>
  </owl:DatatypeProperty>
  <owl:DatatypeProperty rdf:about="http://example.org/onto/prop/google_clouddeploy_deploy_policy_terraform_labels">
    <rdfs:label>terraform_labels</rdfs:label>
    <rdfs:comment>The combination of labels configured directly on the resource
 and default labels configured on the provider.</rdfs:comment>
    <rdfs:domain rdf:resource="http://example.org/onto/class/google_clouddeploy_deploy_policy"/>
    <rdfs:range rdf:resource="http://www.w3.org/2001/XMLSchema#string"/>
  </owl:DatatypeProperty>
  <owl:DatatypeProperty rdf:about="http://example.org/onto/prop/google_clouddeploy_deploy_policy_uid">
    <rdfs:label>uid</rdfs:label>
    <rdfs:comment>Output only. Unique identifier of the 'DeployPolicy'.</rdfs:comment>
    <rdfs:domain rdf:resource="http://example.org/onto/class/google_clouddeploy_deploy_policy"/>
    <rdfs:range rdf:resource="http://www.w3.org/2001/XMLSchema#string"/>
  </owl:DatatypeProperty>
  <owl:DatatypeProperty rdf:about="http://example.org/onto/prop/google_clouddeploy_deploy_policy_update_time">
    <rdfs:label>update_time</rdfs:label>
    <rdfs:comment>Output only. Time at which the DeployPolicy was updated.</rdfs:comment>
    <rdfs:domain rdf:resource="http://example.org/onto/class/google_clouddeploy_deploy_policy"/>
    <rdfs:range rdf:resource="http://www.w3.org/2001/XMLSchema#string"/>
  </owl:DatatypeProperty>
  <owl:DatatypeProperty rdf:about="http://example.org/onto/prop/google_clouddeploy_deploy_policy_actions">
    <rdfs:label>actions</rdfs:label>
    <rdfs:comment>Rollout actions to be restricted as part of the policy. If left empty, all actions will be restricted. Possible values: ["ADVANCE", "APPROVE", "CANCEL", "CREATE", "IGNORE_JOB", "RETRY_JOB", "ROLLBACK", "TERMINATE_JOBRUN"]</rdfs:comment>
    <rdfs:domain rdf:resource="http://example.org/onto/class/google_clouddeploy_deploy_policy"/>
    <rdfs:range rdf:resource="http://www.w3.org/2001/XMLSchema#string"/>
  </owl:DatatypeProperty>
  <owl:DatatypeProperty rdf:about="http://example.org/onto/prop/google_clouddeploy_deploy_policy_id">
    <rdfs:label>id</rdfs:label>
    <rdfs:comment>ID of the rule. This id must be unique in the 'DeployPolicy' resource to which this rule belongs. The format is 'a-z{0,62}'.</rdfs:comment>
    <rdfs:domain rdf:resource="http://example.org/onto/class/google_clouddeploy_deploy_policy"/>
    <rdfs:range rdf:resource="http://www.w3.org/2001/XMLSchema#string"/>
  </owl:DatatypeProperty>
  <owl:DatatypeProperty rdf:about="http://example.org/onto/prop/google_clouddeploy_deploy_policy_invokers">
    <rdfs:label>invokers</rdfs:label>
    <rdfs:comment>What invoked the action. If left empty, all invoker types will be restricted. Possible values: ["USER", "DEPLOY_AUTOMATION"]</rdfs:comment>
    <rdfs:domain rdf:resource="http://example.org/onto/class/google_clouddeploy_deploy_policy"/>
    <rdfs:range rdf:resource="http://www.w3.org/2001/XMLSchema#string"/>
  </owl:DatatypeProperty>
  <owl:DatatypeProperty rdf:about="http://example.org/onto/prop/google_clouddeploy_deploy_policy_time_zone">
    <rdfs:label>time_zone</rdfs:label>
    <rdfs:comment>The time zone in IANA format IANA Time Zone Database (e.g. America/New_York).</rdfs:comment>
    <rdfs:domain rdf:resource="http://example.org/onto/class/google_clouddeploy_deploy_policy"/>
    <rdfs:range rdf:resource="http://www.w3.org/2001/XMLSchema#string"/>
  </owl:DatatypeProperty>
  <owl:DatatypeProperty rdf:about="http://example.org/onto/prop/google_clouddeploy_deploy_policy_day">
    <rdfs:label>day</rdfs:label>
    <rdfs:comment>Day of a month. Must be from 1 to 31 and valid for the year and month.</rdfs:comment>
    <rdfs:domain rdf:resource="http://example.org/onto/class/google_clouddeploy_deploy_policy"/>
    <rdfs:range rdf:resource="http://www.w3.org/2001/XMLSchema#string"/>
  </owl:DatatypeProperty>
  <owl:DatatypeProperty rdf:about="http://example.org/onto/prop/google_clouddeploy_deploy_policy_month">
    <rdfs:label>month</rdfs:label>
    <rdfs:comment>Month of a year. Must be from 1 to 12.</rdfs:comment>
    <rdfs:domain rdf:resource="http://example.org/onto/class/google_clouddeploy_deploy_policy"/>
    <rdfs:range rdf:resource="http://www.w3.org/2001/XMLSchema#string"/>
  </owl:DatatypeProperty>
  <owl:DatatypeProperty rdf:about="http://example.org/onto/prop/google_clouddeploy_deploy_policy_year">
    <rdfs:label>year</rdfs:label>
    <rdfs:comment>Year of the date. Must be from 1 to 9999.</rdfs:comment>
    <rdfs:domain rdf:resource="http://example.org/onto/class/google_clouddeploy_deploy_policy"/>
    <rdfs:range rdf:resource="http://www.w3.org/2001/XMLSchema#string"/>
  </owl:DatatypeProperty>
  <owl:DatatypeProperty rdf:about="http://example.org/onto/prop/google_clouddeploy_deploy_policy_hours">
    <rdfs:label>hours</rdfs:label>
    <rdfs:comment>Hours of a day in 24 hour format. Must be greater than or equal to 0 and typically must be less than or equal to 23. An API may choose to allow the value "24:00:00" for scenarios like business closing time.</rdfs:comment>
    <rdfs:domain rdf:resource="http://example.org/onto/class/google_clouddeploy_deploy_policy"/>
    <rdfs:range rdf:resource="http://www.w3.org/2001/XMLSchema#string"/>
  </owl:DatatypeProperty>
  <owl:DatatypeProperty rdf:about="http://example.org/onto/prop/google_clouddeploy_deploy_policy_minutes">
    <rdfs:label>minutes</rdfs:label>
    <rdfs:comment>Minutes of an hour. Must be greater than or equal to 0 and less than or equal to 59.</rdfs:comment>
    <rdfs:domain rdf:resource="http://example.org/onto/class/google_clouddeploy_deploy_policy"/>
    <rdfs:range rdf:resource="http://www.w3.org/2001/XMLSchema#string"/>
  </owl:DatatypeProperty>
  <owl:DatatypeProperty rdf:about="http://example.org/onto/prop/google_clouddeploy_deploy_policy_nanos">
    <rdfs:label>nanos</rdfs:label>
    <rdfs:comment>Fractions of seconds, in nanoseconds. Must be greater than or equal to 0 and less than or equal to 999,999,999.</rdfs:comment>
    <rdfs:domain rdf:resource="http://example.org/onto/class/google_clouddeploy_deploy_policy"/>
    <rdfs:range rdf:resource="http://www.w3.org/2001/XMLSchema#string"/>
  </owl:DatatypeProperty>
  <owl:DatatypeProperty rdf:about="http://example.org/onto/prop/google_clouddeploy_deploy_policy_seconds">
    <rdfs:label>seconds</rdfs:label>
    <rdfs:comment>Seconds of a minute. Must be greater than or equal to 0 and typically must be less than or equal to 59. An API may allow the value 60 if it allows leap-seconds.</rdfs:comment>
    <rdfs:domain rdf:resource="http://example.org/onto/class/google_clouddeploy_deploy_policy"/>
    <rdfs:range rdf:resource="http://www.w3.org/2001/XMLSchema#string"/>
  </owl:DatatypeProperty>
  <owl:DatatypeProperty rdf:about="http://example.org/onto/prop/google_clouddeploy_deploy_policy_day">
    <rdfs:label>day</rdfs:label>
    <rdfs:comment>Day of a month. Must be from 1 to 31 and valid for the year and month, or 0 to specify a year by itself or a year and month where the day isn't significant.</rdfs:comment>
    <rdfs:domain rdf:resource="http://example.org/onto/class/google_clouddeploy_deploy_policy"/>
    <rdfs:range rdf:resource="http://www.w3.org/2001/XMLSchema#string"/>
  </owl:DatatypeProperty>
  <owl:DatatypeProperty rdf:about="http://example.org/onto/prop/google_clouddeploy_deploy_policy_month">
    <rdfs:label>month</rdfs:label>
    <rdfs:comment>Month of a year. Must be from 1 to 12, or 0 to specify a year without a month and day.</rdfs:comment>
    <rdfs:domain rdf:resource="http://example.org/onto/class/google_clouddeploy_deploy_policy"/>
    <rdfs:range rdf:resource="http://www.w3.org/2001/XMLSchema#string"/>
  </owl:DatatypeProperty>
  <owl:DatatypeProperty rdf:about="http://example.org/onto/prop/google_clouddeploy_deploy_policy_year">
    <rdfs:label>year</rdfs:label>
    <rdfs:comment>Year of the date. Must be from 1 to 9999, or 0 to specify a date without a year.</rdfs:comment>
    <rdfs:domain rdf:resource="http://example.org/onto/class/google_clouddeploy_deploy_policy"/>
    <rdfs:range rdf:resource="http://www.w3.org/2001/XMLSchema#string"/>
  </owl:DatatypeProperty>
  <owl:DatatypeProperty rdf:about="http://example.org/onto/prop/google_clouddeploy_deploy_policy_hours">
    <rdfs:label>hours</rdfs:label>
    <rdfs:comment>Hours of a day in 24 hour format. Must be greater than or equal to 0 and typically must be less than or equal to 23. An API may choose to allow the value "24:00:00" for scenarios like business closing time.</rdfs:comment>
    <rdfs:domain rdf:resource="http://example.org/onto/class/google_clouddeploy_deploy_policy"/>
    <rdfs:range rdf:resource="http://www.w3.org/2001/XMLSchema#string"/>
  </owl:DatatypeProperty>
  <owl:DatatypeProperty rdf:about="http://example.org/onto/prop/google_clouddeploy_deploy_policy_minutes">
    <rdfs:label>minutes</rdfs:label>
    <rdfs:comment>Minutes of an hour. Must be greater than or equal to 0 and less than or equal to 59.</rdfs:comment>
    <rdfs:domain rdf:resource="http://example.org/onto/class/google_clouddeploy_deploy_policy"/>
    <rdfs:range rdf:resource="http://www.w3.org/2001/XMLSchema#string"/>
  </owl:DatatypeProperty>
  <owl:DatatypeProperty rdf:about="http://example.org/onto/prop/google_clouddeploy_deploy_policy_nanos">
    <rdfs:label>nanos</rdfs:label>
    <rdfs:comment>Fractions of seconds, in nanoseconds. Must be greater than or equal to 0 and less than or equal to 999,999,999.</rdfs:comment>
    <rdfs:domain rdf:resource="http://example.org/onto/class/google_clouddeploy_deploy_policy"/>
    <rdfs:range rdf:resource="http://www.w3.org/2001/XMLSchema#string"/>
  </owl:DatatypeProperty>
  <owl:DatatypeProperty rdf:about="http://example.org/onto/prop/google_clouddeploy_deploy_policy_seconds">
    <rdfs:label>seconds</rdfs:label>
    <rdfs:comment>Seconds of a minute. Must be greater than or equal to 0 and typically must be less than or equal to 59. An API may allow the value 60 if it allows leap-seconds.</rdfs:comment>
    <rdfs:domain rdf:resource="http://example.org/onto/class/google_clouddeploy_deploy_policy"/>
    <rdfs:range rdf:resource="http://www.w3.org/2001/XMLSchema#string"/>
  </owl:DatatypeProperty>
  <owl:DatatypeProperty rdf:about="http://example.org/onto/prop/google_clouddeploy_deploy_policy_days_of_week">
    <rdfs:label>days_of_week</rdfs:label>
    <rdfs:comment>Days of week. If left empty, all days of the week will be included. Possible values: ["MONDAY", "TUESDAY", "WEDNESDAY", "THURSDAY", "FRIDAY", "SATURDAY", "SUNDAY"]</rdfs:comment>
    <rdfs:domain rdf:resource="http://example.org/onto/class/google_clouddeploy_deploy_policy"/>
    <rdfs:range rdf:resource="http://www.w3.org/2001/XMLSchema#string"/>
  </owl:DatatypeProperty>
  <owl:DatatypeProperty rdf:about="http://example.org/onto/prop/google_clouddeploy_deploy_policy_hours">
    <rdfs:label>hours</rdfs:label>
    <rdfs:comment>Hours of a day in 24 hour format. Must be greater than or equal to 0 and typically must be less than or equal to 23. An API may choose to allow the value "24:00:00" for scenarios like business closing time.</rdfs:comment>
    <rdfs:domain rdf:resource="http://example.org/onto/class/google_clouddeploy_deploy_policy"/>
    <rdfs:range rdf:resource="http://www.w3.org/2001/XMLSchema#string"/>
  </owl:DatatypeProperty>
  <owl:DatatypeProperty rdf:about="http://example.org/onto/prop/google_clouddeploy_deploy_policy_minutes">
    <rdfs:label>minutes</rdfs:label>
    <rdfs:comment>Minutes of an hour. Must be greater than or equal to 0 and less than or equal to 59.</rdfs:comment>
    <rdfs:domain rdf:resource="http://example.org/onto/class/google_clouddeploy_deploy_policy"/>
    <rdfs:range rdf:resource="http://www.w3.org/2001/XMLSchema#string"/>
  </owl:DatatypeProperty>
  <owl:DatatypeProperty rdf:about="http://example.org/onto/prop/google_clouddeploy_deploy_policy_nanos">
    <rdfs:label>nanos</rdfs:label>
    <rdfs:comment>Fractions of seconds, in nanoseconds. Must be greater than or equal to 0 and less than or equal to 999,999,999.</rdfs:comment>
    <rdfs:domain rdf:resource="http://example.org/onto/class/google_clouddeploy_deploy_policy"/>
    <rdfs:range rdf:resource="http://www.w3.org/2001/XMLSchema#string"/>
  </owl:DatatypeProperty>
  <owl:DatatypeProperty rdf:about="http://example.org/onto/prop/google_clouddeploy_deploy_policy_seconds">
    <rdfs:label>seconds</rdfs:label>
    <rdfs:comment>Seconds of a minute. Must be greater than or equal to 0 and typically must be less than or equal to 59. An API may allow the value 60 if it allows leap-seconds.</rdfs:comment>
    <rdfs:domain rdf:resource="http://example.org/onto/class/google_clouddeploy_deploy_policy"/>
    <rdfs:range rdf:resource="http://www.w3.org/2001/XMLSchema#string"/>
  </owl:DatatypeProperty>
  <owl:DatatypeProperty rdf:about="http://example.org/onto/prop/google_clouddeploy_deploy_policy_hours">
    <rdfs:label>hours</rdfs:label>
    <rdfs:comment>Hours of a day in 24 hour format. Must be greater than or equal to 0 and typically must be less than or equal to 23. An API may choose to allow the value "24:00:00" for scenarios like business closing time.</rdfs:comment>
    <rdfs:domain rdf:resource="http://example.org/onto/class/google_clouddeploy_deploy_policy"/>
    <rdfs:range rdf:resource="http://www.w3.org/2001/XMLSchema#string"/>
  </owl:DatatypeProperty>
  <owl:DatatypeProperty rdf:about="http://example.org/onto/prop/google_clouddeploy_deploy_policy_minutes">
    <rdfs:label>minutes</rdfs:label>
    <rdfs:comment>Minutes of an hour. Must be greater than or equal to 0 and less than or equal to 59.</rdfs:comment>
    <rdfs:domain rdf:resource="http://example.org/onto/class/google_clouddeploy_deploy_policy"/>
    <rdfs:range rdf:resource="http://www.w3.org/2001/XMLSchema#string"/>
  </owl:DatatypeProperty>
  <owl:DatatypeProperty rdf:about="http://example.org/onto/prop/google_clouddeploy_deploy_policy_nanos">
    <rdfs:label>nanos</rdfs:label>
    <rdfs:comment>Fractions of seconds, in nanoseconds. Must be greater than or equal to 0 and less than or equal to 999,999,999.</rdfs:comment>
    <rdfs:domain rdf:resource="http://example.org/onto/class/google_clouddeploy_deploy_policy"/>
    <rdfs:range rdf:resource="http://www.w3.org/2001/XMLSchema#string"/>
  </owl:DatatypeProperty>
  <owl:DatatypeProperty rdf:about="http://example.org/onto/prop/google_clouddeploy_deploy_policy_seconds">
    <rdfs:label>seconds</rdfs:label>
    <rdfs:comment>Seconds of a minute. Must be greater than or equal to 0 and typically must be less than or equal to 59. An API may allow the value 60 if it allows leap-seconds.</rdfs:comment>
    <rdfs:domain rdf:resource="http://example.org/onto/class/google_clouddeploy_deploy_policy"/>
    <rdfs:range rdf:resource="http://www.w3.org/2001/XMLSchema#string"/>
  </owl:DatatypeProperty>
  <owl:DatatypeProperty rdf:about="http://example.org/onto/prop/google_clouddeploy_deploy_policy_id">
    <rdfs:label>id</rdfs:label>
    <rdfs:comment>ID of the DeliveryPipeline. The value of this field could be one of the following:
- The last segment of a pipeline name
- "*", all delivery pipelines in a location</rdfs:comment>
    <rdfs:domain rdf:resource="http://example.org/onto/class/google_clouddeploy_deploy_policy"/>
    <rdfs:range rdf:resource="http://www.w3.org/2001/XMLSchema#string"/>
  </owl:DatatypeProperty>
  <owl:DatatypeProperty rdf:about="http://example.org/onto/prop/google_clouddeploy_deploy_policy_labels">
    <rdfs:label>labels</rdfs:label>
    <rdfs:comment>DeliveryPipeline labels.</rdfs:comment>
    <rdfs:domain rdf:resource="http://example.org/onto/class/google_clouddeploy_deploy_policy"/>
    <rdfs:range rdf:resource="http://www.w3.org/2001/XMLSchema#string"/>
  </owl:DatatypeProperty>
  <owl:DatatypeProperty rdf:about="http://example.org/onto/prop/google_clouddeploy_deploy_policy_id">
    <rdfs:label>id</rdfs:label>
    <rdfs:comment>ID of the 'Target'. The value of this field could be one of the following: * The last segment of a target name. It only needs the ID to determine which target is being referred to * "*", all targets in a location.</rdfs:comment>
    <rdfs:domain rdf:resource="http://example.org/onto/class/google_clouddeploy_deploy_policy"/>
    <rdfs:range rdf:resource="http://www.w3.org/2001/XMLSchema#string"/>
  </owl:DatatypeProperty>
  <owl:DatatypeProperty rdf:about="http://example.org/onto/prop/google_clouddeploy_deploy_policy_labels">
    <rdfs:label>labels</rdfs:label>
    <rdfs:comment>Target labels.</rdfs:comment>
    <rdfs:domain rdf:resource="http://example.org/onto/class/google_clouddeploy_deploy_policy"/>
    <rdfs:range rdf:resource="http://www.w3.org/2001/XMLSchema#string"/>
  </owl:DatatypeProperty>
  <owl:DatatypeProperty rdf:about="http://example.org/onto/prop/google_clouddeploy_deploy_policy_create">
    <rdfs:label>create</rdfs:label>
    <rdfs:domain rdf:resource="http://example.org/onto/class/google_clouddeploy_deploy_policy"/>
    <rdfs:range rdf:resource="http://www.w3.org/2001/XMLSchema#string"/>
  </owl:DatatypeProperty>
  <owl:DatatypeProperty rdf:about="http://example.org/onto/prop/google_clouddeploy_deploy_policy_delete">
    <rdfs:label>delete</rdfs:label>
    <rdfs:domain rdf:resource="http://example.org/onto/class/google_clouddeploy_deploy_policy"/>
    <rdfs:range rdf:resource="http://www.w3.org/2001/XMLSchema#string"/>
  </owl:DatatypeProperty>
  <owl:DatatypeProperty rdf:about="http://example.org/onto/prop/google_clouddeploy_deploy_policy_update">
    <rdfs:label>update</rdfs:label>
    <rdfs:domain rdf:resource="http://example.org/onto/class/google_clouddeploy_deploy_policy"/>
    <rdfs:range rdf:resource="http://www.w3.org/2001/XMLSchema#string"/>
  </owl:DatatypeProperty>
</rdf:RDF>
