<?xml version="1.0" encoding="UTF-8"?>
<rdf:RDF
  xmlns:rdf="http://www.w3.org/1999/02/22-rdf-syntax-ns#"
  xmlns:rdfs="http://www.w3.org/2000/01/rdf-schema#"
  xmlns:owl="http://www.w3.org/2002/07/owl#"
  xmlns:xsd="http://www.w3.org/2001/XMLSchema#"
  xml:base="http://example.org/onto/">
  <owl:Class rdf:about="http://example.org/onto/class/google_spanner_instance_partition">
    <rdfs:label>google_spanner_instance_partition</rdfs:label>
    <rdfs:comment>#
#     ***     AUTO GENERATED CODE    ***    Type: MMv1     ***
#
# ----------------------------------------------------------------------------
#
#     This code is generated by Magic Modules using the following:
#
#     Configuration: https:#github.com/GoogleCloudPlatform/magic-modules/tree/main/mmv1/products/spanner/InstancePartition.yaml
#     Template:      https:#github.com/GoogleCloudPlatform/magic-modules/tree/main/mmv1/templates/terraform/resource.html.markdown.tmpl
#
#     DO NOT EDIT this file directly. Any changes made to this file will be
#     overwritten during the next generation cycle.
#
# ----------------------------------------------------------------------------
subcategory: "Cloud Spanner"
description: |-
  A Cloud Spanner instance partition is a unit of Cloud Spanner database capacity
  that can be used to partition data and processing capacity within an instance.
---</rdfs:comment>
  </owl:Class>
  <owl:DatatypeProperty rdf:about="http://example.org/onto/prop/google_spanner_instance_partition_config">
    <rdfs:label>config</rdfs:label>
    <rdfs:comment>The name of the instance partition's configuration (similar to a region) which
defines the geographic placement and replication of data in this instance partition.</rdfs:comment>
    <rdfs:domain rdf:resource="http://example.org/onto/class/google_spanner_instance_partition"/>
    <rdfs:range rdf:resource="http://www.w3.org/2001/XMLSchema#string"/>
  </owl:DatatypeProperty>
  <owl:DatatypeProperty rdf:about="http://example.org/onto/prop/google_spanner_instance_partition_display_name">
    <rdfs:label>display_name</rdfs:label>
    <rdfs:comment>The descriptive name for this instance partition as it appears in UIs.
Must be unique per project and between 4 and 30 characters in length.</rdfs:comment>
    <rdfs:domain rdf:resource="http://example.org/onto/class/google_spanner_instance_partition"/>
    <rdfs:range rdf:resource="http://www.w3.org/2001/XMLSchema#string"/>
  </owl:DatatypeProperty>
  <owl:DatatypeProperty rdf:about="http://example.org/onto/prop/google_spanner_instance_partition_id">
    <rdfs:label>id</rdfs:label>
    <rdfs:domain rdf:resource="http://example.org/onto/class/google_spanner_instance_partition"/>
    <rdfs:range rdf:resource="http://www.w3.org/2001/XMLSchema#string"/>
  </owl:DatatypeProperty>
  <owl:DatatypeProperty rdf:about="http://example.org/onto/prop/google_spanner_instance_partition_instance">
    <rdfs:label>instance</rdfs:label>
    <rdfs:comment>The instance to create the instance partition in.</rdfs:comment>
    <rdfs:domain rdf:resource="http://example.org/onto/class/google_spanner_instance_partition"/>
    <rdfs:range rdf:resource="http://www.w3.org/2001/XMLSchema#string"/>
  </owl:DatatypeProperty>
  <owl:DatatypeProperty rdf:about="http://example.org/onto/prop/google_spanner_instance_partition_name">
    <rdfs:label>name</rdfs:label>
    <rdfs:comment>A unique identifier for the instance partition, which cannot be changed after
the instance partition is created. The name must be between 2 and 64 characters
and match the regular expression [a-z][a-z0-9\\-]{0,61}[a-z0-9].</rdfs:comment>
    <rdfs:domain rdf:resource="http://example.org/onto/class/google_spanner_instance_partition"/>
    <rdfs:range rdf:resource="http://www.w3.org/2001/XMLSchema#string"/>
  </owl:DatatypeProperty>
  <owl:DatatypeProperty rdf:about="http://example.org/onto/prop/google_spanner_instance_partition_node_count">
    <rdfs:label>node_count</rdfs:label>
    <rdfs:comment>The number of nodes allocated to this instance partition. One node equals
1000 processing units. Exactly one of either node_count or processing_units
must be present.</rdfs:comment>
    <rdfs:domain rdf:resource="http://example.org/onto/class/google_spanner_instance_partition"/>
    <rdfs:range rdf:resource="http://www.w3.org/2001/XMLSchema#string"/>
  </owl:DatatypeProperty>
  <owl:DatatypeProperty rdf:about="http://example.org/onto/prop/google_spanner_instance_partition_processing_units">
    <rdfs:label>processing_units</rdfs:label>
    <rdfs:comment>The number of processing units allocated to this instance partition.
Exactly one of either node_count or processing_units must be present.</rdfs:comment>
    <rdfs:domain rdf:resource="http://example.org/onto/class/google_spanner_instance_partition"/>
    <rdfs:range rdf:resource="http://www.w3.org/2001/XMLSchema#string"/>
  </owl:DatatypeProperty>
  <owl:DatatypeProperty rdf:about="http://example.org/onto/prop/google_spanner_instance_partition_project">
    <rdfs:label>project</rdfs:label>
    <rdfs:domain rdf:resource="http://example.org/onto/class/google_spanner_instance_partition"/>
    <rdfs:range rdf:resource="http://www.w3.org/2001/XMLSchema#string"/>
  </owl:DatatypeProperty>
  <owl:DatatypeProperty rdf:about="http://example.org/onto/prop/google_spanner_instance_partition_state">
    <rdfs:label>state</rdfs:label>
    <rdfs:comment>The current instance partition state. Possible values are:
CREATING: The instance partition is being created. Resources are being
allocated for the instance partition.
READY: The instance partition has been allocated resources and is ready for use.</rdfs:comment>
    <rdfs:domain rdf:resource="http://example.org/onto/class/google_spanner_instance_partition"/>
    <rdfs:range rdf:resource="http://www.w3.org/2001/XMLSchema#string"/>
  </owl:DatatypeProperty>
  <owl:DatatypeProperty rdf:about="http://example.org/onto/prop/google_spanner_instance_partition_create">
    <rdfs:label>create</rdfs:label>
    <rdfs:domain rdf:resource="http://example.org/onto/class/google_spanner_instance_partition"/>
    <rdfs:range rdf:resource="http://www.w3.org/2001/XMLSchema#string"/>
  </owl:DatatypeProperty>
  <owl:DatatypeProperty rdf:about="http://example.org/onto/prop/google_spanner_instance_partition_delete">
    <rdfs:label>delete</rdfs:label>
    <rdfs:domain rdf:resource="http://example.org/onto/class/google_spanner_instance_partition"/>
    <rdfs:range rdf:resource="http://www.w3.org/2001/XMLSchema#string"/>
  </owl:DatatypeProperty>
  <owl:DatatypeProperty rdf:about="http://example.org/onto/prop/google_spanner_instance_partition_update">
    <rdfs:label>update</rdfs:label>
    <rdfs:domain rdf:resource="http://example.org/onto/class/google_spanner_instance_partition"/>
    <rdfs:range rdf:resource="http://www.w3.org/2001/XMLSchema#string"/>
  </owl:DatatypeProperty>
</rdf:RDF>
