<?xml version="1.0" encoding="UTF-8"?>
<rdf:RDF
  xmlns:rdf="http://www.w3.org/1999/02/22-rdf-syntax-ns#"
  xmlns:rdfs="http://www.w3.org/2000/01/rdf-schema#"
  xmlns:owl="http://www.w3.org/2002/07/owl#"
  xmlns:xsd="http://www.w3.org/2001/XMLSchema#"
  xml:base="http://example.org/onto/">
  <owl:Class rdf:about="http://example.org/onto/class/google_data_pipeline_pipeline">
    <rdfs:label>google_data_pipeline_pipeline</rdfs:label>
    <rdfs:comment>#
#     ***     AUTO GENERATED CODE    ***    Type: MMv1     ***
#
# ----------------------------------------------------------------------------
#
#     This code is generated by Magic Modules using the following:
#
#     Configuration: https:#github.com/GoogleCloudPlatform/magic-modules/tree/main/mmv1/products/datapipeline/Pipeline.yaml
#     Template:      https:#github.com/GoogleCloudPlatform/magic-modules/tree/main/mmv1/templates/terraform/resource.html.markdown.tmpl
#
#     DO NOT EDIT this file directly. Any changes made to this file will be
#     overwritten during the next generation cycle.
#
# ----------------------------------------------------------------------------
subcategory: "DataPipeline"
description: |-
  The main pipeline entity and all the necessary metadata for launching and managing linked jobs.
---</rdfs:comment>
  </owl:Class>
  <owl:DatatypeProperty rdf:about="http://example.org/onto/prop/google_data_pipeline_pipeline_create_time">
    <rdfs:label>create_time</rdfs:label>
    <rdfs:comment>The timestamp when the pipeline was initially created. Set by the Data Pipelines service.
A timestamp in RFC3339 UTC "Zulu" format, with nanosecond resolution and up to nine fractional digits. Examples: "2014-10-02T15:01:23Z" and "2014-10-02T15:01:23.045123456Z".</rdfs:comment>
    <rdfs:domain rdf:resource="http://example.org/onto/class/google_data_pipeline_pipeline"/>
    <rdfs:range rdf:resource="http://www.w3.org/2001/XMLSchema#string"/>
  </owl:DatatypeProperty>
  <owl:DatatypeProperty rdf:about="http://example.org/onto/prop/google_data_pipeline_pipeline_display_name">
    <rdfs:label>display_name</rdfs:label>
    <rdfs:comment>The display name of the pipeline. It can contain only letters ([A-Za-z]), numbers ([0-9]), hyphens (-), and underscores (_).</rdfs:comment>
    <rdfs:domain rdf:resource="http://example.org/onto/class/google_data_pipeline_pipeline"/>
    <rdfs:range rdf:resource="http://www.w3.org/2001/XMLSchema#string"/>
  </owl:DatatypeProperty>
  <owl:DatatypeProperty rdf:about="http://example.org/onto/prop/google_data_pipeline_pipeline_id">
    <rdfs:label>id</rdfs:label>
    <rdfs:domain rdf:resource="http://example.org/onto/class/google_data_pipeline_pipeline"/>
    <rdfs:range rdf:resource="http://www.w3.org/2001/XMLSchema#string"/>
  </owl:DatatypeProperty>
  <owl:DatatypeProperty rdf:about="http://example.org/onto/prop/google_data_pipeline_pipeline_job_count">
    <rdfs:label>job_count</rdfs:label>
    <rdfs:comment>Number of jobs.</rdfs:comment>
    <rdfs:domain rdf:resource="http://example.org/onto/class/google_data_pipeline_pipeline"/>
    <rdfs:range rdf:resource="http://www.w3.org/2001/XMLSchema#string"/>
  </owl:DatatypeProperty>
  <owl:DatatypeProperty rdf:about="http://example.org/onto/prop/google_data_pipeline_pipeline_last_update_time">
    <rdfs:label>last_update_time</rdfs:label>
    <rdfs:comment>The timestamp when the pipeline was last modified. Set by the Data Pipelines service.
A timestamp in RFC3339 UTC "Zulu" format, with nanosecond resolution and up to nine fractional digits. Examples: "2014-10-02T15:01:23Z" and "2014-10-02T15:01:23.045123456Z".</rdfs:comment>
    <rdfs:domain rdf:resource="http://example.org/onto/class/google_data_pipeline_pipeline"/>
    <rdfs:range rdf:resource="http://www.w3.org/2001/XMLSchema#string"/>
  </owl:DatatypeProperty>
  <owl:DatatypeProperty rdf:about="http://example.org/onto/prop/google_data_pipeline_pipeline_name">
    <rdfs:label>name</rdfs:label>
    <rdfs:comment>"The pipeline name. For example': 'projects/PROJECT_ID/locations/LOCATION_ID/pipelines/PIPELINE_ID."
"- PROJECT_ID can contain letters ([A-Za-z]), numbers ([0-9]), hyphens (-), colons (:), and periods (.). For more information, see Identifying projects."
"LOCATION_ID is the canonical ID for the pipeline's location. The list of available locations can be obtained by calling google.cloud.location.Locations.ListLocations. Note that the Data Pipelines service is not available in all regions. It depends on Cloud Scheduler, an App Engine application, so it's only available in App Engine regions."
"PIPELINE_ID is the ID of the pipeline. Must be unique for the selected project and location."</rdfs:comment>
    <rdfs:domain rdf:resource="http://example.org/onto/class/google_data_pipeline_pipeline"/>
    <rdfs:range rdf:resource="http://www.w3.org/2001/XMLSchema#string"/>
  </owl:DatatypeProperty>
  <owl:DatatypeProperty rdf:about="http://example.org/onto/prop/google_data_pipeline_pipeline_pipeline_sources">
    <rdfs:label>pipeline_sources</rdfs:label>
    <rdfs:comment>The sources of the pipeline (for example, Dataplex). The keys and values are set by the corresponding sources during pipeline creation.
An object containing a list of "key": value pairs. Example: { "name": "wrench", "mass": "1.3kg", "count": "3" }.</rdfs:comment>
    <rdfs:domain rdf:resource="http://example.org/onto/class/google_data_pipeline_pipeline"/>
    <rdfs:range rdf:resource="http://www.w3.org/2001/XMLSchema#string"/>
  </owl:DatatypeProperty>
  <owl:DatatypeProperty rdf:about="http://example.org/onto/prop/google_data_pipeline_pipeline_project">
    <rdfs:label>project</rdfs:label>
    <rdfs:domain rdf:resource="http://example.org/onto/class/google_data_pipeline_pipeline"/>
    <rdfs:range rdf:resource="http://www.w3.org/2001/XMLSchema#string"/>
  </owl:DatatypeProperty>
  <owl:DatatypeProperty rdf:about="http://example.org/onto/prop/google_data_pipeline_pipeline_region">
    <rdfs:label>region</rdfs:label>
    <rdfs:comment>A reference to the region</rdfs:comment>
    <rdfs:domain rdf:resource="http://example.org/onto/class/google_data_pipeline_pipeline"/>
    <rdfs:range rdf:resource="http://www.w3.org/2001/XMLSchema#string"/>
  </owl:DatatypeProperty>
  <owl:DatatypeProperty rdf:about="http://example.org/onto/prop/google_data_pipeline_pipeline_scheduler_service_account_email">
    <rdfs:label>scheduler_service_account_email</rdfs:label>
    <rdfs:comment>Optional. A service account email to be used with the Cloud Scheduler job. If not specified, the default compute engine service account will be used.</rdfs:comment>
    <rdfs:domain rdf:resource="http://example.org/onto/class/google_data_pipeline_pipeline"/>
    <rdfs:range rdf:resource="http://www.w3.org/2001/XMLSchema#string"/>
  </owl:DatatypeProperty>
  <owl:DatatypeProperty rdf:about="http://example.org/onto/prop/google_data_pipeline_pipeline_state">
    <rdfs:label>state</rdfs:label>
    <rdfs:comment>The state of the pipeline. When the pipeline is created, the state is set to 'PIPELINE_STATE_ACTIVE' by default. State changes can be requested by setting the state to stopping, paused, or resuming. State cannot be changed through pipelines.patch requests.
https://cloud.google.com/dataflow/docs/reference/data-pipelines/rest/v1/projects.locations.pipelines#state Possible values: ["STATE_UNSPECIFIED", "STATE_RESUMING", "STATE_ACTIVE", "STATE_STOPPING", "STATE_ARCHIVED", "STATE_PAUSED"]</rdfs:comment>
    <rdfs:domain rdf:resource="http://example.org/onto/class/google_data_pipeline_pipeline"/>
    <rdfs:range rdf:resource="http://www.w3.org/2001/XMLSchema#string"/>
  </owl:DatatypeProperty>
  <owl:DatatypeProperty rdf:about="http://example.org/onto/prop/google_data_pipeline_pipeline_type">
    <rdfs:label>type</rdfs:label>
    <rdfs:comment>The type of the pipeline. This field affects the scheduling of the pipeline and the type of metrics to show for the pipeline.
https://cloud.google.com/dataflow/docs/reference/data-pipelines/rest/v1/projects.locations.pipelines#pipelinetype Possible values: ["PIPELINE_TYPE_UNSPECIFIED", "PIPELINE_TYPE_BATCH", "PIPELINE_TYPE_STREAMING"]</rdfs:comment>
    <rdfs:domain rdf:resource="http://example.org/onto/class/google_data_pipeline_pipeline"/>
    <rdfs:range rdf:resource="http://www.w3.org/2001/XMLSchema#string"/>
  </owl:DatatypeProperty>
  <owl:DatatypeProperty rdf:about="http://example.org/onto/prop/google_data_pipeline_pipeline_next_job_time">
    <rdfs:label>next_job_time</rdfs:label>
    <rdfs:comment>When the next Scheduler job is going to run.
A timestamp in RFC3339 UTC "Zulu" format, with nanosecond resolution and up to nine fractional digits. Examples: "2014-10-02T15:01:23Z" and "2014-10-02T15:01:23.045123456Z".</rdfs:comment>
    <rdfs:domain rdf:resource="http://example.org/onto/class/google_data_pipeline_pipeline"/>
    <rdfs:range rdf:resource="http://www.w3.org/2001/XMLSchema#string"/>
  </owl:DatatypeProperty>
  <owl:DatatypeProperty rdf:about="http://example.org/onto/prop/google_data_pipeline_pipeline_schedule">
    <rdfs:label>schedule</rdfs:label>
    <rdfs:comment>Unix-cron format of the schedule. This information is retrieved from the linked Cloud Scheduler.</rdfs:comment>
    <rdfs:domain rdf:resource="http://example.org/onto/class/google_data_pipeline_pipeline"/>
    <rdfs:range rdf:resource="http://www.w3.org/2001/XMLSchema#string"/>
  </owl:DatatypeProperty>
  <owl:DatatypeProperty rdf:about="http://example.org/onto/prop/google_data_pipeline_pipeline_time_zone">
    <rdfs:label>time_zone</rdfs:label>
    <rdfs:comment>Timezone ID. This matches the timezone IDs used by the Cloud Scheduler API. If empty, UTC time is assumed.</rdfs:comment>
    <rdfs:domain rdf:resource="http://example.org/onto/class/google_data_pipeline_pipeline"/>
    <rdfs:range rdf:resource="http://www.w3.org/2001/XMLSchema#string"/>
  </owl:DatatypeProperty>
  <owl:DatatypeProperty rdf:about="http://example.org/onto/prop/google_data_pipeline_pipeline_create">
    <rdfs:label>create</rdfs:label>
    <rdfs:domain rdf:resource="http://example.org/onto/class/google_data_pipeline_pipeline"/>
    <rdfs:range rdf:resource="http://www.w3.org/2001/XMLSchema#string"/>
  </owl:DatatypeProperty>
  <owl:DatatypeProperty rdf:about="http://example.org/onto/prop/google_data_pipeline_pipeline_delete">
    <rdfs:label>delete</rdfs:label>
    <rdfs:domain rdf:resource="http://example.org/onto/class/google_data_pipeline_pipeline"/>
    <rdfs:range rdf:resource="http://www.w3.org/2001/XMLSchema#string"/>
  </owl:DatatypeProperty>
  <owl:DatatypeProperty rdf:about="http://example.org/onto/prop/google_data_pipeline_pipeline_update">
    <rdfs:label>update</rdfs:label>
    <rdfs:domain rdf:resource="http://example.org/onto/class/google_data_pipeline_pipeline"/>
    <rdfs:range rdf:resource="http://www.w3.org/2001/XMLSchema#string"/>
  </owl:DatatypeProperty>
  <owl:DatatypeProperty rdf:about="http://example.org/onto/prop/google_data_pipeline_pipeline_location">
    <rdfs:label>location</rdfs:label>
    <rdfs:comment>The regional endpoint to which to direct the request. For example, us-central1, us-west1.</rdfs:comment>
    <rdfs:domain rdf:resource="http://example.org/onto/class/google_data_pipeline_pipeline"/>
    <rdfs:range rdf:resource="http://www.w3.org/2001/XMLSchema#string"/>
  </owl:DatatypeProperty>
  <owl:DatatypeProperty rdf:about="http://example.org/onto/prop/google_data_pipeline_pipeline_project_id">
    <rdfs:label>project_id</rdfs:label>
    <rdfs:comment>The ID of the Cloud Platform project that the job belongs to.</rdfs:comment>
    <rdfs:domain rdf:resource="http://example.org/onto/class/google_data_pipeline_pipeline"/>
    <rdfs:range rdf:resource="http://www.w3.org/2001/XMLSchema#string"/>
  </owl:DatatypeProperty>
  <owl:DatatypeProperty rdf:about="http://example.org/onto/prop/google_data_pipeline_pipeline_validate_only">
    <rdfs:label>validate_only</rdfs:label>
    <rdfs:comment>If true, the request is validated but not actually executed. Defaults to false.</rdfs:comment>
    <rdfs:domain rdf:resource="http://example.org/onto/class/google_data_pipeline_pipeline"/>
    <rdfs:range rdf:resource="http://www.w3.org/2001/XMLSchema#string"/>
  </owl:DatatypeProperty>
  <owl:DatatypeProperty rdf:about="http://example.org/onto/prop/google_data_pipeline_pipeline_container_spec_gcs_path">
    <rdfs:label>container_spec_gcs_path</rdfs:label>
    <rdfs:comment>Cloud Storage path to a file with a JSON-serialized ContainerSpec as content.</rdfs:comment>
    <rdfs:domain rdf:resource="http://example.org/onto/class/google_data_pipeline_pipeline"/>
    <rdfs:range rdf:resource="http://www.w3.org/2001/XMLSchema#string"/>
  </owl:DatatypeProperty>
  <owl:DatatypeProperty rdf:about="http://example.org/onto/prop/google_data_pipeline_pipeline_job_name">
    <rdfs:label>job_name</rdfs:label>
    <rdfs:comment>The job name to use for the created job. For an update job request, the job name should be the same as the existing running job.</rdfs:comment>
    <rdfs:domain rdf:resource="http://example.org/onto/class/google_data_pipeline_pipeline"/>
    <rdfs:range rdf:resource="http://www.w3.org/2001/XMLSchema#string"/>
  </owl:DatatypeProperty>
  <owl:DatatypeProperty rdf:about="http://example.org/onto/prop/google_data_pipeline_pipeline_launch_options">
    <rdfs:label>launch_options</rdfs:label>
    <rdfs:comment>Launch options for this Flex Template job. This is a common set of options across languages and templates. This should not be used to pass job parameters.
'An object containing a list of "key": value pairs. Example: { "name": "wrench", "mass": "1.3kg", "count": "3" }.'</rdfs:comment>
    <rdfs:domain rdf:resource="http://example.org/onto/class/google_data_pipeline_pipeline"/>
    <rdfs:range rdf:resource="http://www.w3.org/2001/XMLSchema#string"/>
  </owl:DatatypeProperty>
  <owl:DatatypeProperty rdf:about="http://example.org/onto/prop/google_data_pipeline_pipeline_parameters">
    <rdfs:label>parameters</rdfs:label>
    <rdfs:comment>'The parameters for the Flex Template. Example: {"numWorkers":"5"}'
'An object containing a list of "key": value pairs. Example: { "name": "wrench", "mass": "1.3kg", "count": "3" }.'</rdfs:comment>
    <rdfs:domain rdf:resource="http://example.org/onto/class/google_data_pipeline_pipeline"/>
    <rdfs:range rdf:resource="http://www.w3.org/2001/XMLSchema#string"/>
  </owl:DatatypeProperty>
  <owl:DatatypeProperty rdf:about="http://example.org/onto/prop/google_data_pipeline_pipeline_transform_name_mappings">
    <rdfs:label>transform_name_mappings</rdfs:label>
    <rdfs:comment>'Use this to pass transform name mappings for streaming update jobs. Example: {"oldTransformName":"newTransformName",...}'
'An object containing a list of "key": value pairs. Example: { "name": "wrench", "mass": "1.3kg", "count": "3" }.'</rdfs:comment>
    <rdfs:domain rdf:resource="http://example.org/onto/class/google_data_pipeline_pipeline"/>
    <rdfs:range rdf:resource="http://www.w3.org/2001/XMLSchema#string"/>
  </owl:DatatypeProperty>
  <owl:DatatypeProperty rdf:about="http://example.org/onto/prop/google_data_pipeline_pipeline_update">
    <rdfs:label>update</rdfs:label>
    <rdfs:comment>Set this to true if you are sending a request to update a running streaming job. When set, the job name should be the same as the running job.</rdfs:comment>
    <rdfs:domain rdf:resource="http://example.org/onto/class/google_data_pipeline_pipeline"/>
    <rdfs:range rdf:resource="http://www.w3.org/2001/XMLSchema#string"/>
  </owl:DatatypeProperty>
  <owl:DatatypeProperty rdf:about="http://example.org/onto/prop/google_data_pipeline_pipeline_additional_experiments">
    <rdfs:label>additional_experiments</rdfs:label>
    <rdfs:comment>Additional experiment flags for the job.</rdfs:comment>
    <rdfs:domain rdf:resource="http://example.org/onto/class/google_data_pipeline_pipeline"/>
    <rdfs:range rdf:resource="http://www.w3.org/2001/XMLSchema#string"/>
  </owl:DatatypeProperty>
  <owl:DatatypeProperty rdf:about="http://example.org/onto/prop/google_data_pipeline_pipeline_additional_user_labels">
    <rdfs:label>additional_user_labels</rdfs:label>
    <rdfs:comment>Additional user labels to be specified for the job. Keys and values should follow the restrictions specified in the labeling restrictions page. An object containing a list of key/value pairs.
'Example: { "name": "wrench", "mass": "1kg", "count": "3" }.'
'An object containing a list of "key": value pairs. Example: { "name": "wrench", "mass": "1.3kg", "count": "3" }.'</rdfs:comment>
    <rdfs:domain rdf:resource="http://example.org/onto/class/google_data_pipeline_pipeline"/>
    <rdfs:range rdf:resource="http://www.w3.org/2001/XMLSchema#string"/>
  </owl:DatatypeProperty>
  <owl:DatatypeProperty rdf:about="http://example.org/onto/prop/google_data_pipeline_pipeline_enable_streaming_engine">
    <rdfs:label>enable_streaming_engine</rdfs:label>
    <rdfs:comment>Whether to enable Streaming Engine for the job.</rdfs:comment>
    <rdfs:domain rdf:resource="http://example.org/onto/class/google_data_pipeline_pipeline"/>
    <rdfs:range rdf:resource="http://www.w3.org/2001/XMLSchema#string"/>
  </owl:DatatypeProperty>
  <owl:DatatypeProperty rdf:about="http://example.org/onto/prop/google_data_pipeline_pipeline_flexrs_goal">
    <rdfs:label>flexrs_goal</rdfs:label>
    <rdfs:comment>Set FlexRS goal for the job. https://cloud.google.com/dataflow/docs/guides/flexrs
https://cloud.google.com/dataflow/docs/reference/data-pipelines/rest/v1/projects.locations.pipelines#FlexResourceSchedulingGoal Possible values: ["FLEXRS_UNSPECIFIED", "FLEXRS_SPEED_OPTIMIZED", "FLEXRS_COST_OPTIMIZED"]</rdfs:comment>
    <rdfs:domain rdf:resource="http://example.org/onto/class/google_data_pipeline_pipeline"/>
    <rdfs:range rdf:resource="http://www.w3.org/2001/XMLSchema#string"/>
  </owl:DatatypeProperty>
  <owl:DatatypeProperty rdf:about="http://example.org/onto/prop/google_data_pipeline_pipeline_ip_configuration">
    <rdfs:label>ip_configuration</rdfs:label>
    <rdfs:comment>Configuration for VM IPs.
https://cloud.google.com/dataflow/docs/reference/data-pipelines/rest/v1/projects.locations.pipelines#WorkerIPAddressConfiguration Possible values: ["WORKER_IP_UNSPECIFIED", "WORKER_IP_PUBLIC", "WORKER_IP_PRIVATE"]</rdfs:comment>
    <rdfs:domain rdf:resource="http://example.org/onto/class/google_data_pipeline_pipeline"/>
    <rdfs:range rdf:resource="http://www.w3.org/2001/XMLSchema#string"/>
  </owl:DatatypeProperty>
  <owl:DatatypeProperty rdf:about="http://example.org/onto/prop/google_data_pipeline_pipeline_kms_key_name">
    <rdfs:label>kms_key_name</rdfs:label>
    <rdfs:comment>'Name for the Cloud KMS key for the job. The key format is: projects//locations//keyRings//cryptoKeys/'</rdfs:comment>
    <rdfs:domain rdf:resource="http://example.org/onto/class/google_data_pipeline_pipeline"/>
    <rdfs:range rdf:resource="http://www.w3.org/2001/XMLSchema#string"/>
  </owl:DatatypeProperty>
  <owl:DatatypeProperty rdf:about="http://example.org/onto/prop/google_data_pipeline_pipeline_machine_type">
    <rdfs:label>machine_type</rdfs:label>
    <rdfs:comment>The machine type to use for the job. Defaults to the value from the template if not specified.</rdfs:comment>
    <rdfs:domain rdf:resource="http://example.org/onto/class/google_data_pipeline_pipeline"/>
    <rdfs:range rdf:resource="http://www.w3.org/2001/XMLSchema#string"/>
  </owl:DatatypeProperty>
  <owl:DatatypeProperty rdf:about="http://example.org/onto/prop/google_data_pipeline_pipeline_max_workers">
    <rdfs:label>max_workers</rdfs:label>
    <rdfs:comment>The maximum number of Compute Engine instances to be made available to your pipeline during execution, from 1 to 1000.</rdfs:comment>
    <rdfs:domain rdf:resource="http://example.org/onto/class/google_data_pipeline_pipeline"/>
    <rdfs:range rdf:resource="http://www.w3.org/2001/XMLSchema#string"/>
  </owl:DatatypeProperty>
  <owl:DatatypeProperty rdf:about="http://example.org/onto/prop/google_data_pipeline_pipeline_network">
    <rdfs:label>network</rdfs:label>
    <rdfs:comment>Network to which VMs will be assigned. If empty or unspecified, the service will use the network "default".</rdfs:comment>
    <rdfs:domain rdf:resource="http://example.org/onto/class/google_data_pipeline_pipeline"/>
    <rdfs:range rdf:resource="http://www.w3.org/2001/XMLSchema#string"/>
  </owl:DatatypeProperty>
  <owl:DatatypeProperty rdf:about="http://example.org/onto/prop/google_data_pipeline_pipeline_num_workers">
    <rdfs:label>num_workers</rdfs:label>
    <rdfs:comment>The initial number of Compute Engine instances for the job.</rdfs:comment>
    <rdfs:domain rdf:resource="http://example.org/onto/class/google_data_pipeline_pipeline"/>
    <rdfs:range rdf:resource="http://www.w3.org/2001/XMLSchema#string"/>
  </owl:DatatypeProperty>
  <owl:DatatypeProperty rdf:about="http://example.org/onto/prop/google_data_pipeline_pipeline_service_account_email">
    <rdfs:label>service_account_email</rdfs:label>
    <rdfs:comment>The email address of the service account to run the job as.</rdfs:comment>
    <rdfs:domain rdf:resource="http://example.org/onto/class/google_data_pipeline_pipeline"/>
    <rdfs:range rdf:resource="http://www.w3.org/2001/XMLSchema#string"/>
  </owl:DatatypeProperty>
  <owl:DatatypeProperty rdf:about="http://example.org/onto/prop/google_data_pipeline_pipeline_subnetwork">
    <rdfs:label>subnetwork</rdfs:label>
    <rdfs:comment>Subnetwork to which VMs will be assigned, if desired. You can specify a subnetwork using either a complete URL or an abbreviated path. Expected to be of the form "https://www.googleapis.com/compute/v1/projects/HOST_PROJECT_ID/regions/REGION/subnetworks/SUBNETWORK" or "regions/REGION/subnetworks/SUBNETWORK". If the subnetwork is located in a Shared VPC network, you must use the complete URL.</rdfs:comment>
    <rdfs:domain rdf:resource="http://example.org/onto/class/google_data_pipeline_pipeline"/>
    <rdfs:range rdf:resource="http://www.w3.org/2001/XMLSchema#string"/>
  </owl:DatatypeProperty>
  <owl:DatatypeProperty rdf:about="http://example.org/onto/prop/google_data_pipeline_pipeline_temp_location">
    <rdfs:label>temp_location</rdfs:label>
    <rdfs:comment>The Cloud Storage path to use for temporary files. Must be a valid Cloud Storage URL, beginning with gs://.</rdfs:comment>
    <rdfs:domain rdf:resource="http://example.org/onto/class/google_data_pipeline_pipeline"/>
    <rdfs:range rdf:resource="http://www.w3.org/2001/XMLSchema#string"/>
  </owl:DatatypeProperty>
  <owl:DatatypeProperty rdf:about="http://example.org/onto/prop/google_data_pipeline_pipeline_worker_region">
    <rdfs:label>worker_region</rdfs:label>
    <rdfs:comment>The Compute Engine region (https://cloud.google.com/compute/docs/regions-zones/regions-zones) in which worker processing should occur, e.g. "us-west1". Mutually exclusive with workerZone. If neither workerRegion nor workerZone is specified, default to the control plane's region.</rdfs:comment>
    <rdfs:domain rdf:resource="http://example.org/onto/class/google_data_pipeline_pipeline"/>
    <rdfs:range rdf:resource="http://www.w3.org/2001/XMLSchema#string"/>
  </owl:DatatypeProperty>
  <owl:DatatypeProperty rdf:about="http://example.org/onto/prop/google_data_pipeline_pipeline_worker_zone">
    <rdfs:label>worker_zone</rdfs:label>
    <rdfs:comment>The Compute Engine zone (https://cloud.google.com/compute/docs/regions-zones/regions-zones) in which worker processing should occur, e.g. "us-west1-a". Mutually exclusive with workerRegion. If neither workerRegion nor workerZone is specified, a zone in the control plane's region is chosen based on available capacity. If both workerZone and zone are set, workerZone takes precedence.</rdfs:comment>
    <rdfs:domain rdf:resource="http://example.org/onto/class/google_data_pipeline_pipeline"/>
    <rdfs:range rdf:resource="http://www.w3.org/2001/XMLSchema#string"/>
  </owl:DatatypeProperty>
  <owl:DatatypeProperty rdf:about="http://example.org/onto/prop/google_data_pipeline_pipeline_zone">
    <rdfs:label>zone</rdfs:label>
    <rdfs:comment>The Compute Engine availability zone for launching worker instances to run your pipeline. In the future, workerZone will take precedence.</rdfs:comment>
    <rdfs:domain rdf:resource="http://example.org/onto/class/google_data_pipeline_pipeline"/>
    <rdfs:range rdf:resource="http://www.w3.org/2001/XMLSchema#string"/>
  </owl:DatatypeProperty>
  <owl:DatatypeProperty rdf:about="http://example.org/onto/prop/google_data_pipeline_pipeline_gcs_path">
    <rdfs:label>gcs_path</rdfs:label>
    <rdfs:comment>A Cloud Storage path to the template from which to create the job. Must be a valid Cloud Storage URL, beginning with 'gs://'.</rdfs:comment>
    <rdfs:domain rdf:resource="http://example.org/onto/class/google_data_pipeline_pipeline"/>
    <rdfs:range rdf:resource="http://www.w3.org/2001/XMLSchema#string"/>
  </owl:DatatypeProperty>
  <owl:DatatypeProperty rdf:about="http://example.org/onto/prop/google_data_pipeline_pipeline_location">
    <rdfs:label>location</rdfs:label>
    <rdfs:comment>The regional endpoint to which to direct the request.</rdfs:comment>
    <rdfs:domain rdf:resource="http://example.org/onto/class/google_data_pipeline_pipeline"/>
    <rdfs:range rdf:resource="http://www.w3.org/2001/XMLSchema#string"/>
  </owl:DatatypeProperty>
  <owl:DatatypeProperty rdf:about="http://example.org/onto/prop/google_data_pipeline_pipeline_project_id">
    <rdfs:label>project_id</rdfs:label>
    <rdfs:comment>The ID of the Cloud Platform project that the job belongs to.</rdfs:comment>
    <rdfs:domain rdf:resource="http://example.org/onto/class/google_data_pipeline_pipeline"/>
    <rdfs:range rdf:resource="http://www.w3.org/2001/XMLSchema#string"/>
  </owl:DatatypeProperty>
  <owl:DatatypeProperty rdf:about="http://example.org/onto/prop/google_data_pipeline_pipeline_validate_only">
    <rdfs:label>validate_only</rdfs:label>
    <rdfs:domain rdf:resource="http://example.org/onto/class/google_data_pipeline_pipeline"/>
    <rdfs:range rdf:resource="http://www.w3.org/2001/XMLSchema#string"/>
  </owl:DatatypeProperty>
  <owl:DatatypeProperty rdf:about="http://example.org/onto/prop/google_data_pipeline_pipeline_job_name">
    <rdfs:label>job_name</rdfs:label>
    <rdfs:comment>The job name to use for the created job.</rdfs:comment>
    <rdfs:domain rdf:resource="http://example.org/onto/class/google_data_pipeline_pipeline"/>
    <rdfs:range rdf:resource="http://www.w3.org/2001/XMLSchema#string"/>
  </owl:DatatypeProperty>
  <owl:DatatypeProperty rdf:about="http://example.org/onto/prop/google_data_pipeline_pipeline_parameters">
    <rdfs:label>parameters</rdfs:label>
    <rdfs:comment>The runtime parameters to pass to the job.
'An object containing a list of "key": value pairs. Example: { "name": "wrench", "mass": "1.3kg", "count": "3" }.'</rdfs:comment>
    <rdfs:domain rdf:resource="http://example.org/onto/class/google_data_pipeline_pipeline"/>
    <rdfs:range rdf:resource="http://www.w3.org/2001/XMLSchema#string"/>
  </owl:DatatypeProperty>
  <owl:DatatypeProperty rdf:about="http://example.org/onto/prop/google_data_pipeline_pipeline_transform_name_mapping">
    <rdfs:label>transform_name_mapping</rdfs:label>
    <rdfs:comment>Map of transform name prefixes of the job to be replaced to the corresponding name prefixes of the new job. Only applicable when updating a pipeline.
'An object containing a list of "key": value pairs. Example: { "name": "wrench", "mass": "1.3kg", "count": "3" }.'</rdfs:comment>
    <rdfs:domain rdf:resource="http://example.org/onto/class/google_data_pipeline_pipeline"/>
    <rdfs:range rdf:resource="http://www.w3.org/2001/XMLSchema#string"/>
  </owl:DatatypeProperty>
  <owl:DatatypeProperty rdf:about="http://example.org/onto/prop/google_data_pipeline_pipeline_update">
    <rdfs:label>update</rdfs:label>
    <rdfs:comment>If set, replace the existing pipeline with the name specified by jobName with this pipeline, preserving state.</rdfs:comment>
    <rdfs:domain rdf:resource="http://example.org/onto/class/google_data_pipeline_pipeline"/>
    <rdfs:range rdf:resource="http://www.w3.org/2001/XMLSchema#string"/>
  </owl:DatatypeProperty>
  <owl:DatatypeProperty rdf:about="http://example.org/onto/prop/google_data_pipeline_pipeline_additional_experiments">
    <rdfs:label>additional_experiments</rdfs:label>
    <rdfs:comment>Additional experiment flags for the job.</rdfs:comment>
    <rdfs:domain rdf:resource="http://example.org/onto/class/google_data_pipeline_pipeline"/>
    <rdfs:range rdf:resource="http://www.w3.org/2001/XMLSchema#string"/>
  </owl:DatatypeProperty>
  <owl:DatatypeProperty rdf:about="http://example.org/onto/prop/google_data_pipeline_pipeline_additional_user_labels">
    <rdfs:label>additional_user_labels</rdfs:label>
    <rdfs:comment>Additional user labels to be specified for the job. Keys and values should follow the restrictions specified in the labeling restrictions page. An object containing a list of key/value pairs.
'Example: { "name": "wrench", "mass": "1kg", "count": "3" }.'
'An object containing a list of "key": value pairs. Example: { "name": "wrench", "mass": "1.3kg", "count": "3" }.'</rdfs:comment>
    <rdfs:domain rdf:resource="http://example.org/onto/class/google_data_pipeline_pipeline"/>
    <rdfs:range rdf:resource="http://www.w3.org/2001/XMLSchema#string"/>
  </owl:DatatypeProperty>
  <owl:DatatypeProperty rdf:about="http://example.org/onto/prop/google_data_pipeline_pipeline_bypass_temp_dir_validation">
    <rdfs:label>bypass_temp_dir_validation</rdfs:label>
    <rdfs:comment>Whether to bypass the safety checks for the job's temporary directory. Use with caution.</rdfs:comment>
    <rdfs:domain rdf:resource="http://example.org/onto/class/google_data_pipeline_pipeline"/>
    <rdfs:range rdf:resource="http://www.w3.org/2001/XMLSchema#string"/>
  </owl:DatatypeProperty>
  <owl:DatatypeProperty rdf:about="http://example.org/onto/prop/google_data_pipeline_pipeline_enable_streaming_engine">
    <rdfs:label>enable_streaming_engine</rdfs:label>
    <rdfs:comment>Whether to enable Streaming Engine for the job.</rdfs:comment>
    <rdfs:domain rdf:resource="http://example.org/onto/class/google_data_pipeline_pipeline"/>
    <rdfs:range rdf:resource="http://www.w3.org/2001/XMLSchema#string"/>
  </owl:DatatypeProperty>
  <owl:DatatypeProperty rdf:about="http://example.org/onto/prop/google_data_pipeline_pipeline_ip_configuration">
    <rdfs:label>ip_configuration</rdfs:label>
    <rdfs:comment>Configuration for VM IPs.
https://cloud.google.com/dataflow/docs/reference/data-pipelines/rest/v1/projects.locations.pipelines#WorkerIPAddressConfiguration Possible values: ["WORKER_IP_UNSPECIFIED", "WORKER_IP_PUBLIC", "WORKER_IP_PRIVATE"]</rdfs:comment>
    <rdfs:domain rdf:resource="http://example.org/onto/class/google_data_pipeline_pipeline"/>
    <rdfs:range rdf:resource="http://www.w3.org/2001/XMLSchema#string"/>
  </owl:DatatypeProperty>
  <owl:DatatypeProperty rdf:about="http://example.org/onto/prop/google_data_pipeline_pipeline_kms_key_name">
    <rdfs:label>kms_key_name</rdfs:label>
    <rdfs:comment>'Name for the Cloud KMS key for the job. The key format is: projects//locations//keyRings//cryptoKeys/'</rdfs:comment>
    <rdfs:domain rdf:resource="http://example.org/onto/class/google_data_pipeline_pipeline"/>
    <rdfs:range rdf:resource="http://www.w3.org/2001/XMLSchema#string"/>
  </owl:DatatypeProperty>
  <owl:DatatypeProperty rdf:about="http://example.org/onto/prop/google_data_pipeline_pipeline_machine_type">
    <rdfs:label>machine_type</rdfs:label>
    <rdfs:comment>The machine type to use for the job. Defaults to the value from the template if not specified.</rdfs:comment>
    <rdfs:domain rdf:resource="http://example.org/onto/class/google_data_pipeline_pipeline"/>
    <rdfs:range rdf:resource="http://www.w3.org/2001/XMLSchema#string"/>
  </owl:DatatypeProperty>
  <owl:DatatypeProperty rdf:about="http://example.org/onto/prop/google_data_pipeline_pipeline_max_workers">
    <rdfs:label>max_workers</rdfs:label>
    <rdfs:comment>The maximum number of Compute Engine instances to be made available to your pipeline during execution, from 1 to 1000.</rdfs:comment>
    <rdfs:domain rdf:resource="http://example.org/onto/class/google_data_pipeline_pipeline"/>
    <rdfs:range rdf:resource="http://www.w3.org/2001/XMLSchema#string"/>
  </owl:DatatypeProperty>
  <owl:DatatypeProperty rdf:about="http://example.org/onto/prop/google_data_pipeline_pipeline_network">
    <rdfs:label>network</rdfs:label>
    <rdfs:comment>Network to which VMs will be assigned. If empty or unspecified, the service will use the network "default".</rdfs:comment>
    <rdfs:domain rdf:resource="http://example.org/onto/class/google_data_pipeline_pipeline"/>
    <rdfs:range rdf:resource="http://www.w3.org/2001/XMLSchema#string"/>
  </owl:DatatypeProperty>
  <owl:DatatypeProperty rdf:about="http://example.org/onto/prop/google_data_pipeline_pipeline_num_workers">
    <rdfs:label>num_workers</rdfs:label>
    <rdfs:comment>The initial number of Compute Engine instances for the job.</rdfs:comment>
    <rdfs:domain rdf:resource="http://example.org/onto/class/google_data_pipeline_pipeline"/>
    <rdfs:range rdf:resource="http://www.w3.org/2001/XMLSchema#string"/>
  </owl:DatatypeProperty>
  <owl:DatatypeProperty rdf:about="http://example.org/onto/prop/google_data_pipeline_pipeline_service_account_email">
    <rdfs:label>service_account_email</rdfs:label>
    <rdfs:comment>The email address of the service account to run the job as.</rdfs:comment>
    <rdfs:domain rdf:resource="http://example.org/onto/class/google_data_pipeline_pipeline"/>
    <rdfs:range rdf:resource="http://www.w3.org/2001/XMLSchema#string"/>
  </owl:DatatypeProperty>
  <owl:DatatypeProperty rdf:about="http://example.org/onto/prop/google_data_pipeline_pipeline_subnetwork">
    <rdfs:label>subnetwork</rdfs:label>
    <rdfs:comment>Subnetwork to which VMs will be assigned, if desired. You can specify a subnetwork using either a complete URL or an abbreviated path. Expected to be of the form "https://www.googleapis.com/compute/v1/projects/HOST_PROJECT_ID/regions/REGION/subnetworks/SUBNETWORK" or "regions/REGION/subnetworks/SUBNETWORK". If the subnetwork is located in a Shared VPC network, you must use the complete URL.</rdfs:comment>
    <rdfs:domain rdf:resource="http://example.org/onto/class/google_data_pipeline_pipeline"/>
    <rdfs:range rdf:resource="http://www.w3.org/2001/XMLSchema#string"/>
  </owl:DatatypeProperty>
  <owl:DatatypeProperty rdf:about="http://example.org/onto/prop/google_data_pipeline_pipeline_temp_location">
    <rdfs:label>temp_location</rdfs:label>
    <rdfs:comment>The Cloud Storage path to use for temporary files. Must be a valid Cloud Storage URL, beginning with gs://.</rdfs:comment>
    <rdfs:domain rdf:resource="http://example.org/onto/class/google_data_pipeline_pipeline"/>
    <rdfs:range rdf:resource="http://www.w3.org/2001/XMLSchema#string"/>
  </owl:DatatypeProperty>
  <owl:DatatypeProperty rdf:about="http://example.org/onto/prop/google_data_pipeline_pipeline_worker_region">
    <rdfs:label>worker_region</rdfs:label>
    <rdfs:comment>The Compute Engine region (https://cloud.google.com/compute/docs/regions-zones/regions-zones) in which worker processing should occur, e.g. "us-west1". Mutually exclusive with workerZone. If neither workerRegion nor workerZone is specified, default to the control plane's region.</rdfs:comment>
    <rdfs:domain rdf:resource="http://example.org/onto/class/google_data_pipeline_pipeline"/>
    <rdfs:range rdf:resource="http://www.w3.org/2001/XMLSchema#string"/>
  </owl:DatatypeProperty>
  <owl:DatatypeProperty rdf:about="http://example.org/onto/prop/google_data_pipeline_pipeline_worker_zone">
    <rdfs:label>worker_zone</rdfs:label>
    <rdfs:comment>The Compute Engine zone (https://cloud.google.com/compute/docs/regions-zones/regions-zones) in which worker processing should occur, e.g. "us-west1-a". Mutually exclusive with workerRegion. If neither workerRegion nor workerZone is specified, a zone in the control plane's region is chosen based on available capacity. If both workerZone and zone are set, workerZone takes precedence.</rdfs:comment>
    <rdfs:domain rdf:resource="http://example.org/onto/class/google_data_pipeline_pipeline"/>
    <rdfs:range rdf:resource="http://www.w3.org/2001/XMLSchema#string"/>
  </owl:DatatypeProperty>
  <owl:DatatypeProperty rdf:about="http://example.org/onto/prop/google_data_pipeline_pipeline_zone">
    <rdfs:label>zone</rdfs:label>
    <rdfs:comment>The Compute Engine availability zone for launching worker instances to run your pipeline. In the future, workerZone will take precedence.</rdfs:comment>
    <rdfs:domain rdf:resource="http://example.org/onto/class/google_data_pipeline_pipeline"/>
    <rdfs:range rdf:resource="http://www.w3.org/2001/XMLSchema#string"/>
  </owl:DatatypeProperty>
</rdf:RDF>
