<?xml version="1.0" encoding="UTF-8"?>
<rdf:RDF
  xmlns:rdf="http://www.w3.org/1999/02/22-rdf-syntax-ns#"
  xmlns:rdfs="http://www.w3.org/2000/01/rdf-schema#"
  xmlns:owl="http://www.w3.org/2002/07/owl#"
  xmlns:xsd="http://www.w3.org/2001/XMLSchema#"
  xml:base="http://example.org/onto/">
  <owl:Class rdf:about="http://example.org/onto/class/google_apikeys_key">
    <rdfs:label>google_apikeys_key</rdfs:label>
    <rdfs:comment>#
#     ***     AUTO GENERATED CODE    ***    Type: DCL     ***
#
# ----------------------------------------------------------------------------
#
#     This file is managed by Magic Modules (https:#github.com/GoogleCloudPlatform/magic-modules)
#     and is based on the DCL (https:#github.com/GoogleCloudPlatform/declarative-resource-client-library).
#     Changes will need to be made to the DCL or Magic Modules instead of here.
#
#     We are not currently able to accept contributions to this file. If changes
#     are required, please file an issue at https:#github.com/hashicorp/terraform-provider-google/issues/new/choose
#
# ----------------------------------------------------------------------------
subcategory: "Apikeys"
description: |-
  The Apikeys Key resource
---</rdfs:comment>
  </owl:Class>
  <owl:DatatypeProperty rdf:about="http://example.org/onto/prop/google_apikeys_key_display_name">
    <rdfs:label>display_name</rdfs:label>
    <rdfs:comment>Human-readable display name of this API key. Modifiable by user.</rdfs:comment>
    <rdfs:domain rdf:resource="http://example.org/onto/class/google_apikeys_key"/>
    <rdfs:range rdf:resource="http://www.w3.org/2001/XMLSchema#string"/>
  </owl:DatatypeProperty>
  <owl:DatatypeProperty rdf:about="http://example.org/onto/prop/google_apikeys_key_id">
    <rdfs:label>id</rdfs:label>
    <rdfs:domain rdf:resource="http://example.org/onto/class/google_apikeys_key"/>
    <rdfs:range rdf:resource="http://www.w3.org/2001/XMLSchema#string"/>
  </owl:DatatypeProperty>
  <owl:DatatypeProperty rdf:about="http://example.org/onto/prop/google_apikeys_key_key_string">
    <rdfs:label>key_string</rdfs:label>
    <rdfs:comment>Output only. An encrypted and signed value held by this key. This field can be accessed only through the `GetKeyString` method.</rdfs:comment>
    <rdfs:domain rdf:resource="http://example.org/onto/class/google_apikeys_key"/>
    <rdfs:range rdf:resource="http://www.w3.org/2001/XMLSchema#string"/>
  </owl:DatatypeProperty>
  <owl:DatatypeProperty rdf:about="http://example.org/onto/prop/google_apikeys_key_name">
    <rdfs:label>name</rdfs:label>
    <rdfs:comment>The resource name of the key. The name must be unique within the project, must conform with RFC-1034, is restricted to lower-cased letters, and has a maximum length of 63 characters. In another word, the name must match the regular expression: `[a-z]([a-z0-9-]{0,61}[a-z0-9])?`.</rdfs:comment>
    <rdfs:domain rdf:resource="http://example.org/onto/class/google_apikeys_key"/>
    <rdfs:range rdf:resource="http://www.w3.org/2001/XMLSchema#string"/>
  </owl:DatatypeProperty>
  <owl:DatatypeProperty rdf:about="http://example.org/onto/prop/google_apikeys_key_project">
    <rdfs:label>project</rdfs:label>
    <rdfs:comment>The project for the resource</rdfs:comment>
    <rdfs:domain rdf:resource="http://example.org/onto/class/google_apikeys_key"/>
    <rdfs:range rdf:resource="http://www.w3.org/2001/XMLSchema#string"/>
  </owl:DatatypeProperty>
  <owl:DatatypeProperty rdf:about="http://example.org/onto/prop/google_apikeys_key_service_account_email">
    <rdfs:label>service_account_email</rdfs:label>
    <rdfs:comment>The email of the service account the key is bound to. If this field is specified, the key is a service account bound key and auth enabled. See [Documentation](https://cloud.devsite.corp.google.com/docs/authentication/api-keys?#api-keys-bound-sa) for more details.</rdfs:comment>
    <rdfs:domain rdf:resource="http://example.org/onto/class/google_apikeys_key"/>
    <rdfs:range rdf:resource="http://www.w3.org/2001/XMLSchema#string"/>
  </owl:DatatypeProperty>
  <owl:DatatypeProperty rdf:about="http://example.org/onto/prop/google_apikeys_key_uid">
    <rdfs:label>uid</rdfs:label>
    <rdfs:comment>Output only. Unique id in UUID4 format.</rdfs:comment>
    <rdfs:domain rdf:resource="http://example.org/onto/class/google_apikeys_key"/>
    <rdfs:range rdf:resource="http://www.w3.org/2001/XMLSchema#string"/>
  </owl:DatatypeProperty>
  <owl:DatatypeProperty rdf:about="http://example.org/onto/prop/google_apikeys_key_package_name">
    <rdfs:label>package_name</rdfs:label>
    <rdfs:comment>The package name of the application.</rdfs:comment>
    <rdfs:domain rdf:resource="http://example.org/onto/class/google_apikeys_key"/>
    <rdfs:range rdf:resource="http://www.w3.org/2001/XMLSchema#string"/>
  </owl:DatatypeProperty>
  <owl:DatatypeProperty rdf:about="http://example.org/onto/prop/google_apikeys_key_sha1_fingerprint">
    <rdfs:label>sha1_fingerprint</rdfs:label>
    <rdfs:comment>The SHA1 fingerprint of the application. For example, both sha1 formats are acceptable : DA:39:A3:EE:5E:6B:4B:0D:32:55:BF:EF:95:60:18:90:AF:D8:07:09 or DA39A3EE5E6B4B0D3255BFEF95601890AFD80709. Output format is the latter.</rdfs:comment>
    <rdfs:domain rdf:resource="http://example.org/onto/class/google_apikeys_key"/>
    <rdfs:range rdf:resource="http://www.w3.org/2001/XMLSchema#string"/>
  </owl:DatatypeProperty>
  <owl:DatatypeProperty rdf:about="http://example.org/onto/prop/google_apikeys_key_methods">
    <rdfs:label>methods</rdfs:label>
    <rdfs:comment>Optional. List of one or more methods that can be called. If empty, all methods for the service are allowed. A wildcard (*) can be used as the last symbol. Valid examples: `google.cloud.translate.v2.TranslateService.GetSupportedLanguage` `TranslateText` `Get*` `translate.googleapis.com.Get*`</rdfs:comment>
    <rdfs:domain rdf:resource="http://example.org/onto/class/google_apikeys_key"/>
    <rdfs:range rdf:resource="http://www.w3.org/2001/XMLSchema#string"/>
  </owl:DatatypeProperty>
  <owl:DatatypeProperty rdf:about="http://example.org/onto/prop/google_apikeys_key_service">
    <rdfs:label>service</rdfs:label>
    <rdfs:comment>The service for this restriction. It should be the canonical service name, for example: `translate.googleapis.com`. You can use `gcloud services list` to get a list of services that are enabled in the project.</rdfs:comment>
    <rdfs:domain rdf:resource="http://example.org/onto/class/google_apikeys_key"/>
    <rdfs:range rdf:resource="http://www.w3.org/2001/XMLSchema#string"/>
  </owl:DatatypeProperty>
  <owl:DatatypeProperty rdf:about="http://example.org/onto/prop/google_apikeys_key_allowed_referrers">
    <rdfs:label>allowed_referrers</rdfs:label>
    <rdfs:comment>A list of regular expressions for the referrer URLs that are allowed to make API calls with this key.</rdfs:comment>
    <rdfs:domain rdf:resource="http://example.org/onto/class/google_apikeys_key"/>
    <rdfs:range rdf:resource="http://www.w3.org/2001/XMLSchema#string"/>
  </owl:DatatypeProperty>
  <owl:DatatypeProperty rdf:about="http://example.org/onto/prop/google_apikeys_key_allowed_bundle_ids">
    <rdfs:label>allowed_bundle_ids</rdfs:label>
    <rdfs:comment>A list of bundle IDs that are allowed when making API calls with this key.</rdfs:comment>
    <rdfs:domain rdf:resource="http://example.org/onto/class/google_apikeys_key"/>
    <rdfs:range rdf:resource="http://www.w3.org/2001/XMLSchema#string"/>
  </owl:DatatypeProperty>
  <owl:DatatypeProperty rdf:about="http://example.org/onto/prop/google_apikeys_key_allowed_ips">
    <rdfs:label>allowed_ips</rdfs:label>
    <rdfs:comment>A list of the caller IP addresses that are allowed to make API calls with this key.</rdfs:comment>
    <rdfs:domain rdf:resource="http://example.org/onto/class/google_apikeys_key"/>
    <rdfs:range rdf:resource="http://www.w3.org/2001/XMLSchema#string"/>
  </owl:DatatypeProperty>
  <owl:DatatypeProperty rdf:about="http://example.org/onto/prop/google_apikeys_key_create">
    <rdfs:label>create</rdfs:label>
    <rdfs:domain rdf:resource="http://example.org/onto/class/google_apikeys_key"/>
    <rdfs:range rdf:resource="http://www.w3.org/2001/XMLSchema#string"/>
  </owl:DatatypeProperty>
  <owl:DatatypeProperty rdf:about="http://example.org/onto/prop/google_apikeys_key_delete">
    <rdfs:label>delete</rdfs:label>
    <rdfs:domain rdf:resource="http://example.org/onto/class/google_apikeys_key"/>
    <rdfs:range rdf:resource="http://www.w3.org/2001/XMLSchema#string"/>
  </owl:DatatypeProperty>
  <owl:DatatypeProperty rdf:about="http://example.org/onto/prop/google_apikeys_key_update">
    <rdfs:label>update</rdfs:label>
    <rdfs:domain rdf:resource="http://example.org/onto/class/google_apikeys_key"/>
    <rdfs:range rdf:resource="http://www.w3.org/2001/XMLSchema#string"/>
  </owl:DatatypeProperty>
</rdf:RDF>
