<?xml version="1.0" encoding="UTF-8"?>
<rdf:RDF
  xmlns:rdf="http://www.w3.org/1999/02/22-rdf-syntax-ns#"
  xmlns:rdfs="http://www.w3.org/2000/01/rdf-schema#"
  xmlns:owl="http://www.w3.org/2002/07/owl#"
  xmlns:xsd="http://www.w3.org/2001/XMLSchema#"
  xml:base="http://example.org/onto/">
  <owl:Class rdf:about="http://example.org/onto/class/google_compute_backend_service">
    <rdfs:label>google_compute_backend_service</rdfs:label>
    <rdfs:comment>#
#     ***     AUTO GENERATED CODE    ***    Type: MMv1     ***
#
# ----------------------------------------------------------------------------
#
#     This code is generated by Magic Modules using the following:
#
#     Configuration: https:#github.com/GoogleCloudPlatform/magic-modules/tree/main/mmv1/products/compute/BackendService.yaml
#     Template:      https:#github.com/GoogleCloudPlatform/magic-modules/tree/main/mmv1/templates/terraform/resource.html.markdown.tmpl
#
#     DO NOT EDIT this file directly. Any changes made to this file will be
#     overwritten during the next generation cycle.
#
# ----------------------------------------------------------------------------
subcategory: "Compute Engine"
description: |-
  A Backend Service defines a group of virtual machines that will serve
  traffic for load balancing.
---</rdfs:comment>
  </owl:Class>
  <owl:DatatypeProperty rdf:about="http://example.org/onto/prop/google_compute_backend_service_affinity_cookie_ttl_sec">
    <rdfs:label>affinity_cookie_ttl_sec</rdfs:label>
    <rdfs:comment>Lifetime of cookies in seconds if session_affinity is
GENERATED_COOKIE. If set to 0, the cookie is non-persistent and lasts
only until the end of the browser session (or equivalent). The
maximum allowed value for TTL is one day.

When the load balancing scheme is INTERNAL, this field is not used.</rdfs:comment>
    <rdfs:domain rdf:resource="http://example.org/onto/class/google_compute_backend_service"/>
    <rdfs:range rdf:resource="http://www.w3.org/2001/XMLSchema#string"/>
  </owl:DatatypeProperty>
  <owl:DatatypeProperty rdf:about="http://example.org/onto/prop/google_compute_backend_service_compression_mode">
    <rdfs:label>compression_mode</rdfs:label>
    <rdfs:comment>Compress text responses using Brotli or gzip compression, based on the client's Accept-Encoding header. Possible values: ["AUTOMATIC", "DISABLED"]</rdfs:comment>
    <rdfs:domain rdf:resource="http://example.org/onto/class/google_compute_backend_service"/>
    <rdfs:range rdf:resource="http://www.w3.org/2001/XMLSchema#string"/>
  </owl:DatatypeProperty>
  <owl:DatatypeProperty rdf:about="http://example.org/onto/prop/google_compute_backend_service_connection_draining_timeout_sec">
    <rdfs:label>connection_draining_timeout_sec</rdfs:label>
    <rdfs:comment>Time for which instance will be drained (not accept new
connections, but still work to finish started).</rdfs:comment>
    <rdfs:domain rdf:resource="http://example.org/onto/class/google_compute_backend_service"/>
    <rdfs:range rdf:resource="http://www.w3.org/2001/XMLSchema#string"/>
  </owl:DatatypeProperty>
  <owl:DatatypeProperty rdf:about="http://example.org/onto/prop/google_compute_backend_service_creation_timestamp">
    <rdfs:label>creation_timestamp</rdfs:label>
    <rdfs:comment>Creation timestamp in RFC3339 text format.</rdfs:comment>
    <rdfs:domain rdf:resource="http://example.org/onto/class/google_compute_backend_service"/>
    <rdfs:range rdf:resource="http://www.w3.org/2001/XMLSchema#string"/>
  </owl:DatatypeProperty>
  <owl:DatatypeProperty rdf:about="http://example.org/onto/prop/google_compute_backend_service_custom_request_headers">
    <rdfs:label>custom_request_headers</rdfs:label>
    <rdfs:comment>Headers that the HTTP/S load balancer should add to proxied
requests.</rdfs:comment>
    <rdfs:domain rdf:resource="http://example.org/onto/class/google_compute_backend_service"/>
    <rdfs:range rdf:resource="http://www.w3.org/2001/XMLSchema#string"/>
  </owl:DatatypeProperty>
  <owl:DatatypeProperty rdf:about="http://example.org/onto/prop/google_compute_backend_service_custom_response_headers">
    <rdfs:label>custom_response_headers</rdfs:label>
    <rdfs:comment>Headers that the HTTP/S load balancer should add to proxied
responses.</rdfs:comment>
    <rdfs:domain rdf:resource="http://example.org/onto/class/google_compute_backend_service"/>
    <rdfs:range rdf:resource="http://www.w3.org/2001/XMLSchema#string"/>
  </owl:DatatypeProperty>
  <owl:DatatypeProperty rdf:about="http://example.org/onto/prop/google_compute_backend_service_description">
    <rdfs:label>description</rdfs:label>
    <rdfs:comment>An optional description of this resource.</rdfs:comment>
    <rdfs:domain rdf:resource="http://example.org/onto/class/google_compute_backend_service"/>
    <rdfs:range rdf:resource="http://www.w3.org/2001/XMLSchema#string"/>
  </owl:DatatypeProperty>
  <owl:DatatypeProperty rdf:about="http://example.org/onto/prop/google_compute_backend_service_edge_security_policy">
    <rdfs:label>edge_security_policy</rdfs:label>
    <rdfs:comment>The resource URL for the edge security policy associated with this backend service.</rdfs:comment>
    <rdfs:domain rdf:resource="http://example.org/onto/class/google_compute_backend_service"/>
    <rdfs:range rdf:resource="http://www.w3.org/2001/XMLSchema#string"/>
  </owl:DatatypeProperty>
  <owl:DatatypeProperty rdf:about="http://example.org/onto/prop/google_compute_backend_service_enable_cdn">
    <rdfs:label>enable_cdn</rdfs:label>
    <rdfs:comment>If true, enable Cloud CDN for this BackendService.</rdfs:comment>
    <rdfs:domain rdf:resource="http://example.org/onto/class/google_compute_backend_service"/>
    <rdfs:range rdf:resource="http://www.w3.org/2001/XMLSchema#string"/>
  </owl:DatatypeProperty>
  <owl:DatatypeProperty rdf:about="http://example.org/onto/prop/google_compute_backend_service_external_managed_migration_state">
    <rdfs:label>external_managed_migration_state</rdfs:label>
    <rdfs:comment>Specifies the canary migration state. Possible values are PREPARE, TEST_BY_PERCENTAGE, and
TEST_ALL_TRAFFIC.

To begin the migration from EXTERNAL to EXTERNAL_MANAGED, the state must be changed to
PREPARE. The state must be changed to TEST_ALL_TRAFFIC before the loadBalancingScheme can be
changed to EXTERNAL_MANAGED. Optionally, the TEST_BY_PERCENTAGE state can be used to migrate
traffic by percentage using externalManagedMigrationTestingPercentage.

Rolling back a migration requires the states to be set in reverse order. So changing the
scheme from EXTERNAL_MANAGED to EXTERNAL requires the state to be set to TEST_ALL_TRAFFIC at
the same time. Optionally, the TEST_BY_PERCENTAGE state can be used to migrate some traffic
back to EXTERNAL or PREPARE can be used to migrate all traffic back to EXTERNAL. Possible values: ["PREPARE", "TEST_BY_PERCENTAGE", "TEST_ALL_TRAFFIC"]</rdfs:comment>
    <rdfs:domain rdf:resource="http://example.org/onto/class/google_compute_backend_service"/>
    <rdfs:range rdf:resource="http://www.w3.org/2001/XMLSchema#string"/>
  </owl:DatatypeProperty>
  <owl:DatatypeProperty rdf:about="http://example.org/onto/prop/google_compute_backend_service_external_managed_migration_testing_percentage">
    <rdfs:label>external_managed_migration_testing_percentage</rdfs:label>
    <rdfs:comment>Determines the fraction of requests that should be processed by the Global external
Application Load Balancer.

The value of this field must be in the range [0, 100].

Session affinity options will slightly affect this routing behavior, for more details,
see: Session Affinity.

This value can only be set if the loadBalancingScheme in the backend service is set to
EXTERNAL (when using the Classic ALB) and the migration state is TEST_BY_PERCENTAGE.</rdfs:comment>
    <rdfs:domain rdf:resource="http://example.org/onto/class/google_compute_backend_service"/>
    <rdfs:range rdf:resource="http://www.w3.org/2001/XMLSchema#string"/>
  </owl:DatatypeProperty>
  <owl:DatatypeProperty rdf:about="http://example.org/onto/prop/google_compute_backend_service_fingerprint">
    <rdfs:label>fingerprint</rdfs:label>
    <rdfs:comment>Fingerprint of this resource. A hash of the contents stored in this
object. This field is used in optimistic locking.</rdfs:comment>
    <rdfs:domain rdf:resource="http://example.org/onto/class/google_compute_backend_service"/>
    <rdfs:range rdf:resource="http://www.w3.org/2001/XMLSchema#string"/>
  </owl:DatatypeProperty>
  <owl:DatatypeProperty rdf:about="http://example.org/onto/prop/google_compute_backend_service_generated_id">
    <rdfs:label>generated_id</rdfs:label>
    <rdfs:comment>The unique identifier for the resource. This identifier is defined by the server.</rdfs:comment>
    <rdfs:domain rdf:resource="http://example.org/onto/class/google_compute_backend_service"/>
    <rdfs:range rdf:resource="http://www.w3.org/2001/XMLSchema#string"/>
  </owl:DatatypeProperty>
  <owl:DatatypeProperty rdf:about="http://example.org/onto/prop/google_compute_backend_service_health_checks">
    <rdfs:label>health_checks</rdfs:label>
    <rdfs:comment>The set of URLs to the HttpHealthCheck or HttpsHealthCheck resource
for health checking this BackendService. Currently at most one health
check can be specified.

A health check must be specified unless the backend service uses an internet
or serverless NEG as a backend.

For internal load balancing, a URL to a HealthCheck resource must be specified instead.</rdfs:comment>
    <rdfs:domain rdf:resource="http://example.org/onto/class/google_compute_backend_service"/>
    <rdfs:range rdf:resource="http://www.w3.org/2001/XMLSchema#string"/>
  </owl:DatatypeProperty>
  <owl:DatatypeProperty rdf:about="http://example.org/onto/prop/google_compute_backend_service_id">
    <rdfs:label>id</rdfs:label>
    <rdfs:domain rdf:resource="http://example.org/onto/class/google_compute_backend_service"/>
    <rdfs:range rdf:resource="http://www.w3.org/2001/XMLSchema#string"/>
  </owl:DatatypeProperty>
  <owl:DatatypeProperty rdf:about="http://example.org/onto/prop/google_compute_backend_service_ip_address_selection_policy">
    <rdfs:label>ip_address_selection_policy</rdfs:label>
    <rdfs:comment>Specifies preference of traffic to the backend (from the proxy and from the client for proxyless gRPC). Possible values: ["IPV4_ONLY", "PREFER_IPV6", "IPV6_ONLY"]</rdfs:comment>
    <rdfs:domain rdf:resource="http://example.org/onto/class/google_compute_backend_service"/>
    <rdfs:range rdf:resource="http://www.w3.org/2001/XMLSchema#string"/>
  </owl:DatatypeProperty>
  <owl:DatatypeProperty rdf:about="http://example.org/onto/prop/google_compute_backend_service_load_balancing_scheme">
    <rdfs:label>load_balancing_scheme</rdfs:label>
    <rdfs:comment>Indicates whether the backend service will be used with internal or
external load balancing. A backend service created for one type of
load balancing cannot be used with the other. For more information, refer to
[Choosing a load balancer](https://cloud.google.com/load-balancing/docs/backend-service). Default value: "EXTERNAL" Possible values: ["EXTERNAL", "INTERNAL_SELF_MANAGED", "INTERNAL_MANAGED", "EXTERNAL_MANAGED"]</rdfs:comment>
    <rdfs:domain rdf:resource="http://example.org/onto/class/google_compute_backend_service"/>
    <rdfs:range rdf:resource="http://www.w3.org/2001/XMLSchema#string"/>
  </owl:DatatypeProperty>
  <owl:DatatypeProperty rdf:about="http://example.org/onto/prop/google_compute_backend_service_locality_lb_policy">
    <rdfs:label>locality_lb_policy</rdfs:label>
    <rdfs:comment>The load balancing algorithm used within the scope of the locality.
The possible values are:

* 'ROUND_ROBIN': This is a simple policy in which each healthy backend
                 is selected in round robin order.

* 'LEAST_REQUEST': An O(1) algorithm which selects two random healthy
                   hosts and picks the host which has fewer active requests.

* 'RING_HASH': The ring/modulo hash load balancer implements consistent
               hashing to backends. The algorithm has the property that the
               addition/removal of a host from a set of N hosts only affects
               1/N of the requests.

* 'RANDOM': The load balancer selects a random healthy host.

* 'ORIGINAL_DESTINATION': Backend host is selected based on the client
                          connection metadata, i.e., connections are opened
                          to the same address as the destination address of
                          the incoming connection before the connection
                          was redirected to the load balancer.

* 'MAGLEV': used as a drop in replacement for the ring hash load balancer.
            Maglev is not as stable as ring hash but has faster table lookup
            build times and host selection times. For more information about
            Maglev, refer to https://ai.google/research/pubs/pub44824

* 'WEIGHTED_MAGLEV': Per-instance weighted Load Balancing via health check
                     reported weights. Only applicable to loadBalancingScheme
                     EXTERNAL. If set, the Backend Service must
                     configure a non legacy HTTP-based Health Check, and
                     health check replies are expected to contain
                     non-standard HTTP response header field
                     X-Load-Balancing-Endpoint-Weight to specify the
                     per-instance weights. If set, Load Balancing is weight
                     based on the per-instance weights reported in the last
                     processed health check replies, as long as every
                     instance either reported a valid weight or had
                     UNAVAILABLE_WEIGHT. Otherwise, Load Balancing remains
                     equal-weight.

* 'WEIGHTED_ROUND_ROBIN': Per-endpoint weighted round-robin Load Balancing using weights computed
                          from Backend reported Custom Metrics. If set, the Backend Service
                          responses are expected to contain non-standard HTTP response header field
                          X-Endpoint-Load-Metrics. The reported metrics
                          to use for computing the weights are specified via the
                          backends[].customMetrics fields.

locality_lb_policy is applicable to either:

* A regional backend service with the service_protocol set to HTTP, HTTPS, HTTP2 or H2C,
  and loadBalancingScheme set to INTERNAL_MANAGED.
* A global backend service with the load_balancing_scheme set to INTERNAL_SELF_MANAGED.
* A regional backend service with loadBalancingScheme set to EXTERNAL (External Network
  Load Balancing). Only MAGLEV and WEIGHTED_MAGLEV values are possible for External
  Network Load Balancing. The default is MAGLEV.

If session_affinity is not NONE, and locality_lb_policy is not set to MAGLEV, WEIGHTED_MAGLEV,
or RING_HASH, session affinity settings will not take effect.

Only ROUND_ROBIN and RING_HASH are supported when the backend service is referenced
by a URL map that is bound to target gRPC proxy that has validate_for_proxyless
field set to true. Possible values: ["ROUND_ROBIN", "LEAST_REQUEST", "RING_HASH", "RANDOM", "ORIGINAL_DESTINATION", "MAGLEV", "WEIGHTED_MAGLEV", "WEIGHTED_ROUND_ROBIN"]</rdfs:comment>
    <rdfs:domain rdf:resource="http://example.org/onto/class/google_compute_backend_service"/>
    <rdfs:range rdf:resource="http://www.w3.org/2001/XMLSchema#string"/>
  </owl:DatatypeProperty>
  <owl:DatatypeProperty rdf:about="http://example.org/onto/prop/google_compute_backend_service_name">
    <rdfs:label>name</rdfs:label>
    <rdfs:comment>Name of the resource. Provided by the client when the resource is
created. The name must be 1-63 characters long, and comply with
RFC1035. Specifically, the name must be 1-63 characters long and match
the regular expression '[a-z]([-a-z0-9]*[a-z0-9])?' which means the
first character must be a lowercase letter, and all following
characters must be a dash, lowercase letter, or digit, except the last
character, which cannot be a dash.</rdfs:comment>
    <rdfs:domain rdf:resource="http://example.org/onto/class/google_compute_backend_service"/>
    <rdfs:range rdf:resource="http://www.w3.org/2001/XMLSchema#string"/>
  </owl:DatatypeProperty>
  <owl:DatatypeProperty rdf:about="http://example.org/onto/prop/google_compute_backend_service_port_name">
    <rdfs:label>port_name</rdfs:label>
    <rdfs:comment>Name of backend port. The same name should appear in the instance
groups referenced by this service. Required when the load balancing
scheme is EXTERNAL.</rdfs:comment>
    <rdfs:domain rdf:resource="http://example.org/onto/class/google_compute_backend_service"/>
    <rdfs:range rdf:resource="http://www.w3.org/2001/XMLSchema#string"/>
  </owl:DatatypeProperty>
  <owl:DatatypeProperty rdf:about="http://example.org/onto/prop/google_compute_backend_service_project">
    <rdfs:label>project</rdfs:label>
    <rdfs:domain rdf:resource="http://example.org/onto/class/google_compute_backend_service"/>
    <rdfs:range rdf:resource="http://www.w3.org/2001/XMLSchema#string"/>
  </owl:DatatypeProperty>
  <owl:DatatypeProperty rdf:about="http://example.org/onto/prop/google_compute_backend_service_protocol">
    <rdfs:label>protocol</rdfs:label>
    <rdfs:comment>The protocol this BackendService uses to communicate with backends.
The default is HTTP. Possible values are HTTP, HTTPS, HTTP2, H2C, TCP, SSL, UDP
or GRPC. Refer to the documentation for the load balancers or for Traffic Director
for more information. Must be set to GRPC when the backend service is referenced
by a URL map that is bound to target gRPC proxy. Possible values: ["HTTP", "HTTPS", "HTTP2", "TCP", "SSL", "UDP", "GRPC", "UNSPECIFIED", "H2C"]</rdfs:comment>
    <rdfs:domain rdf:resource="http://example.org/onto/class/google_compute_backend_service"/>
    <rdfs:range rdf:resource="http://www.w3.org/2001/XMLSchema#string"/>
  </owl:DatatypeProperty>
  <owl:DatatypeProperty rdf:about="http://example.org/onto/prop/google_compute_backend_service_security_policy">
    <rdfs:label>security_policy</rdfs:label>
    <rdfs:comment>The security policy associated with this backend service.</rdfs:comment>
    <rdfs:domain rdf:resource="http://example.org/onto/class/google_compute_backend_service"/>
    <rdfs:range rdf:resource="http://www.w3.org/2001/XMLSchema#string"/>
  </owl:DatatypeProperty>
  <owl:DatatypeProperty rdf:about="http://example.org/onto/prop/google_compute_backend_service_self_link">
    <rdfs:label>self_link</rdfs:label>
    <rdfs:domain rdf:resource="http://example.org/onto/class/google_compute_backend_service"/>
    <rdfs:range rdf:resource="http://www.w3.org/2001/XMLSchema#string"/>
  </owl:DatatypeProperty>
  <owl:DatatypeProperty rdf:about="http://example.org/onto/prop/google_compute_backend_service_service_lb_policy">
    <rdfs:label>service_lb_policy</rdfs:label>
    <rdfs:comment>URL to networkservices.ServiceLbPolicy resource.
Can only be set if load balancing scheme is EXTERNAL, EXTERNAL_MANAGED, INTERNAL_MANAGED or INTERNAL_SELF_MANAGED and the scope is global.</rdfs:comment>
    <rdfs:domain rdf:resource="http://example.org/onto/class/google_compute_backend_service"/>
    <rdfs:range rdf:resource="http://www.w3.org/2001/XMLSchema#string"/>
  </owl:DatatypeProperty>
  <owl:DatatypeProperty rdf:about="http://example.org/onto/prop/google_compute_backend_service_session_affinity">
    <rdfs:label>session_affinity</rdfs:label>
    <rdfs:comment>Type of session affinity to use. The default is NONE. Session affinity is
not applicable if the protocol is UDP. Possible values: ["NONE", "CLIENT_IP", "CLIENT_IP_PORT_PROTO", "CLIENT_IP_PROTO", "GENERATED_COOKIE", "HEADER_FIELD", "HTTP_COOKIE", "STRONG_COOKIE_AFFINITY"]</rdfs:comment>
    <rdfs:domain rdf:resource="http://example.org/onto/class/google_compute_backend_service"/>
    <rdfs:range rdf:resource="http://www.w3.org/2001/XMLSchema#string"/>
  </owl:DatatypeProperty>
  <owl:DatatypeProperty rdf:about="http://example.org/onto/prop/google_compute_backend_service_timeout_sec">
    <rdfs:label>timeout_sec</rdfs:label>
    <rdfs:comment>The backend service timeout has a different meaning depending on the type of load balancer.
For more information see, [Backend service settings](https://cloud.google.com/compute/docs/reference/rest/v1/backendServices).
The default is 30 seconds.
The full range of timeout values allowed goes from 1 through 2,147,483,647 seconds.</rdfs:comment>
    <rdfs:domain rdf:resource="http://example.org/onto/class/google_compute_backend_service"/>
    <rdfs:range rdf:resource="http://www.w3.org/2001/XMLSchema#string"/>
  </owl:DatatypeProperty>
  <owl:DatatypeProperty rdf:about="http://example.org/onto/prop/google_compute_backend_service_balancing_mode">
    <rdfs:label>balancing_mode</rdfs:label>
    <rdfs:comment>Specifies the balancing mode for this backend.

For global HTTP(S) or TCP/SSL load balancing, the default is
UTILIZATION. Valid values are UTILIZATION, RATE (for HTTP(S)),
CUSTOM_METRICS (for HTTP(s)) and CONNECTION (for TCP/SSL).

See the [Backend Services Overview](https://cloud.google.com/load-balancing/docs/backend-service#balancing-mode)
for an explanation of load balancing modes. Default value: "UTILIZATION" Possible values: ["UTILIZATION", "RATE", "CONNECTION", "CUSTOM_METRICS"]</rdfs:comment>
    <rdfs:domain rdf:resource="http://example.org/onto/class/google_compute_backend_service"/>
    <rdfs:range rdf:resource="http://www.w3.org/2001/XMLSchema#string"/>
  </owl:DatatypeProperty>
  <owl:DatatypeProperty rdf:about="http://example.org/onto/prop/google_compute_backend_service_capacity_scaler">
    <rdfs:label>capacity_scaler</rdfs:label>
    <rdfs:comment>A multiplier applied to the group's maximum servicing capacity
(based on UTILIZATION, RATE or CONNECTION).

Default value is 1, which means the group will serve up to 100%
of its configured capacity (depending on balancingMode). A
setting of 0 means the group is completely drained, offering
0% of its available Capacity. Valid range is [0.0,1.0].</rdfs:comment>
    <rdfs:domain rdf:resource="http://example.org/onto/class/google_compute_backend_service"/>
    <rdfs:range rdf:resource="http://www.w3.org/2001/XMLSchema#string"/>
  </owl:DatatypeProperty>
  <owl:DatatypeProperty rdf:about="http://example.org/onto/prop/google_compute_backend_service_description">
    <rdfs:label>description</rdfs:label>
    <rdfs:comment>An optional description of this resource.
Provide this property when you create the resource.</rdfs:comment>
    <rdfs:domain rdf:resource="http://example.org/onto/class/google_compute_backend_service"/>
    <rdfs:range rdf:resource="http://www.w3.org/2001/XMLSchema#string"/>
  </owl:DatatypeProperty>
  <owl:DatatypeProperty rdf:about="http://example.org/onto/prop/google_compute_backend_service_group">
    <rdfs:label>group</rdfs:label>
    <rdfs:comment>The fully-qualified URL of an Instance Group or Network Endpoint
Group resource. In case of instance group this defines the list
of instances that serve traffic. Member virtual machine
instances from each instance group must live in the same zone as
the instance group itself. No two backends in a backend service
are allowed to use same Instance Group resource.

For Network Endpoint Groups this defines list of endpoints. All
endpoints of Network Endpoint Group must be hosted on instances
located in the same zone as the Network Endpoint Group.

Backend services cannot mix Instance Group and
Network Endpoint Group backends.

Note that you must specify an Instance Group or Network Endpoint
Group resource using the fully-qualified URL, rather than a
partial URL.</rdfs:comment>
    <rdfs:domain rdf:resource="http://example.org/onto/class/google_compute_backend_service"/>
    <rdfs:range rdf:resource="http://www.w3.org/2001/XMLSchema#string"/>
  </owl:DatatypeProperty>
  <owl:DatatypeProperty rdf:about="http://example.org/onto/prop/google_compute_backend_service_max_connections">
    <rdfs:label>max_connections</rdfs:label>
    <rdfs:comment>The max number of simultaneous connections for the group. Can
be used with either CONNECTION or UTILIZATION balancing modes.

For CONNECTION mode, either maxConnections or one
of maxConnectionsPerInstance or maxConnectionsPerEndpoint,
as appropriate for group type, must be set.</rdfs:comment>
    <rdfs:domain rdf:resource="http://example.org/onto/class/google_compute_backend_service"/>
    <rdfs:range rdf:resource="http://www.w3.org/2001/XMLSchema#string"/>
  </owl:DatatypeProperty>
  <owl:DatatypeProperty rdf:about="http://example.org/onto/prop/google_compute_backend_service_max_connections_per_endpoint">
    <rdfs:label>max_connections_per_endpoint</rdfs:label>
    <rdfs:comment>The max number of simultaneous connections that a single backend
network endpoint can handle. This is used to calculate the
capacity of the group. Can be used in either CONNECTION or
UTILIZATION balancing modes.

For CONNECTION mode, either
maxConnections or maxConnectionsPerEndpoint must be set.</rdfs:comment>
    <rdfs:domain rdf:resource="http://example.org/onto/class/google_compute_backend_service"/>
    <rdfs:range rdf:resource="http://www.w3.org/2001/XMLSchema#string"/>
  </owl:DatatypeProperty>
  <owl:DatatypeProperty rdf:about="http://example.org/onto/prop/google_compute_backend_service_max_connections_per_instance">
    <rdfs:label>max_connections_per_instance</rdfs:label>
    <rdfs:comment>The max number of simultaneous connections that a single
backend instance can handle. This is used to calculate the
capacity of the group. Can be used in either CONNECTION or
UTILIZATION balancing modes.

For CONNECTION mode, either maxConnections or
maxConnectionsPerInstance must be set.</rdfs:comment>
    <rdfs:domain rdf:resource="http://example.org/onto/class/google_compute_backend_service"/>
    <rdfs:range rdf:resource="http://www.w3.org/2001/XMLSchema#string"/>
  </owl:DatatypeProperty>
  <owl:DatatypeProperty rdf:about="http://example.org/onto/prop/google_compute_backend_service_max_rate">
    <rdfs:label>max_rate</rdfs:label>
    <rdfs:comment>The max requests per second (RPS) of the group.

Can be used with either RATE or UTILIZATION balancing modes,
but required if RATE mode. For RATE mode, either maxRate or one
of maxRatePerInstance or maxRatePerEndpoint, as appropriate for
group type, must be set.</rdfs:comment>
    <rdfs:domain rdf:resource="http://example.org/onto/class/google_compute_backend_service"/>
    <rdfs:range rdf:resource="http://www.w3.org/2001/XMLSchema#string"/>
  </owl:DatatypeProperty>
  <owl:DatatypeProperty rdf:about="http://example.org/onto/prop/google_compute_backend_service_max_rate_per_endpoint">
    <rdfs:label>max_rate_per_endpoint</rdfs:label>
    <rdfs:comment>The max requests per second (RPS) that a single backend network
endpoint can handle. This is used to calculate the capacity of
the group. Can be used in either balancing mode. For RATE mode,
either maxRate or maxRatePerEndpoint must be set.</rdfs:comment>
    <rdfs:domain rdf:resource="http://example.org/onto/class/google_compute_backend_service"/>
    <rdfs:range rdf:resource="http://www.w3.org/2001/XMLSchema#string"/>
  </owl:DatatypeProperty>
  <owl:DatatypeProperty rdf:about="http://example.org/onto/prop/google_compute_backend_service_max_rate_per_instance">
    <rdfs:label>max_rate_per_instance</rdfs:label>
    <rdfs:comment>The max requests per second (RPS) that a single backend
instance can handle. This is used to calculate the capacity of
the group. Can be used in either balancing mode. For RATE mode,
either maxRate or maxRatePerInstance must be set.</rdfs:comment>
    <rdfs:domain rdf:resource="http://example.org/onto/class/google_compute_backend_service"/>
    <rdfs:range rdf:resource="http://www.w3.org/2001/XMLSchema#string"/>
  </owl:DatatypeProperty>
  <owl:DatatypeProperty rdf:about="http://example.org/onto/prop/google_compute_backend_service_max_utilization">
    <rdfs:label>max_utilization</rdfs:label>
    <rdfs:comment>Used when balancingMode is UTILIZATION. This ratio defines the
CPU utilization target for the group. Valid range is [0.0, 1.0].</rdfs:comment>
    <rdfs:domain rdf:resource="http://example.org/onto/class/google_compute_backend_service"/>
    <rdfs:range rdf:resource="http://www.w3.org/2001/XMLSchema#string"/>
  </owl:DatatypeProperty>
  <owl:DatatypeProperty rdf:about="http://example.org/onto/prop/google_compute_backend_service_preference">
    <rdfs:label>preference</rdfs:label>
    <rdfs:comment>This field indicates whether this backend should be fully utilized before sending traffic to backends
with default preference. This field cannot be set when loadBalancingScheme is set to 'EXTERNAL'. The possible values are:
  - PREFERRED: Backends with this preference level will be filled up to their capacity limits first,
    based on RTT.
  - DEFAULT: If preferred backends don't have enough capacity, backends in this layer would be used and
    traffic would be assigned based on the load balancing algorithm you use. This is the default Possible values: ["PREFERRED", "DEFAULT"]</rdfs:comment>
    <rdfs:domain rdf:resource="http://example.org/onto/class/google_compute_backend_service"/>
    <rdfs:range rdf:resource="http://www.w3.org/2001/XMLSchema#string"/>
  </owl:DatatypeProperty>
  <owl:DatatypeProperty rdf:about="http://example.org/onto/prop/google_compute_backend_service_dry_run">
    <rdfs:label>dry_run</rdfs:label>
    <rdfs:comment>If true, the metric data is collected and reported to Cloud
Monitoring, but is not used for load balancing.</rdfs:comment>
    <rdfs:domain rdf:resource="http://example.org/onto/class/google_compute_backend_service"/>
    <rdfs:range rdf:resource="http://www.w3.org/2001/XMLSchema#string"/>
  </owl:DatatypeProperty>
  <owl:DatatypeProperty rdf:about="http://example.org/onto/prop/google_compute_backend_service_max_utilization">
    <rdfs:label>max_utilization</rdfs:label>
    <rdfs:comment>Optional parameter to define a target utilization for the Custom Metrics
balancing mode. The valid range is <code>[0.0, 1.0]</code>.</rdfs:comment>
    <rdfs:domain rdf:resource="http://example.org/onto/class/google_compute_backend_service"/>
    <rdfs:range rdf:resource="http://www.w3.org/2001/XMLSchema#string"/>
  </owl:DatatypeProperty>
  <owl:DatatypeProperty rdf:about="http://example.org/onto/prop/google_compute_backend_service_name">
    <rdfs:label>name</rdfs:label>
    <rdfs:comment>Name of a custom utilization signal. The name must be 1-64 characters
long and match the regular expression [a-z]([-_.a-z0-9]*[a-z0-9])? which
means the first character must be a lowercase letter, and all following
characters must be a dash, period, underscore, lowercase letter, or
digit, except the last character, which cannot be a dash, period, or
underscore. For usage guidelines, see Custom Metrics balancing mode. This
field can only be used for a global or regional backend service with the
loadBalancingScheme set to <code>EXTERNAL_MANAGED</code>,
<code>INTERNAL_MANAGED</code> <code>INTERNAL_SELF_MANAGED</code>.</rdfs:comment>
    <rdfs:domain rdf:resource="http://example.org/onto/class/google_compute_backend_service"/>
    <rdfs:range rdf:resource="http://www.w3.org/2001/XMLSchema#string"/>
  </owl:DatatypeProperty>
  <owl:DatatypeProperty rdf:about="http://example.org/onto/prop/google_compute_backend_service_cache_mode">
    <rdfs:label>cache_mode</rdfs:label>
    <rdfs:comment>Specifies the cache setting for all responses from this backend.
The possible values are: USE_ORIGIN_HEADERS, FORCE_CACHE_ALL and CACHE_ALL_STATIC Possible values: ["USE_ORIGIN_HEADERS", "FORCE_CACHE_ALL", "CACHE_ALL_STATIC"]</rdfs:comment>
    <rdfs:domain rdf:resource="http://example.org/onto/class/google_compute_backend_service"/>
    <rdfs:range rdf:resource="http://www.w3.org/2001/XMLSchema#string"/>
  </owl:DatatypeProperty>
  <owl:DatatypeProperty rdf:about="http://example.org/onto/prop/google_compute_backend_service_client_ttl">
    <rdfs:label>client_ttl</rdfs:label>
    <rdfs:comment>Specifies the maximum allowed TTL for cached content served by this origin.</rdfs:comment>
    <rdfs:domain rdf:resource="http://example.org/onto/class/google_compute_backend_service"/>
    <rdfs:range rdf:resource="http://www.w3.org/2001/XMLSchema#string"/>
  </owl:DatatypeProperty>
  <owl:DatatypeProperty rdf:about="http://example.org/onto/prop/google_compute_backend_service_default_ttl">
    <rdfs:label>default_ttl</rdfs:label>
    <rdfs:comment>Specifies the default TTL for cached content served by this origin for responses
that do not have an existing valid TTL (max-age or s-max-age).</rdfs:comment>
    <rdfs:domain rdf:resource="http://example.org/onto/class/google_compute_backend_service"/>
    <rdfs:range rdf:resource="http://www.w3.org/2001/XMLSchema#string"/>
  </owl:DatatypeProperty>
  <owl:DatatypeProperty rdf:about="http://example.org/onto/prop/google_compute_backend_service_max_ttl">
    <rdfs:label>max_ttl</rdfs:label>
    <rdfs:comment>Specifies the maximum allowed TTL for cached content served by this origin.</rdfs:comment>
    <rdfs:domain rdf:resource="http://example.org/onto/class/google_compute_backend_service"/>
    <rdfs:range rdf:resource="http://www.w3.org/2001/XMLSchema#string"/>
  </owl:DatatypeProperty>
  <owl:DatatypeProperty rdf:about="http://example.org/onto/prop/google_compute_backend_service_negative_caching">
    <rdfs:label>negative_caching</rdfs:label>
    <rdfs:comment>Negative caching allows per-status code TTLs to be set, in order to apply fine-grained caching for common errors or redirects.</rdfs:comment>
    <rdfs:domain rdf:resource="http://example.org/onto/class/google_compute_backend_service"/>
    <rdfs:range rdf:resource="http://www.w3.org/2001/XMLSchema#string"/>
  </owl:DatatypeProperty>
  <owl:DatatypeProperty rdf:about="http://example.org/onto/prop/google_compute_backend_service_request_coalescing">
    <rdfs:label>request_coalescing</rdfs:label>
    <rdfs:comment>If true then Cloud CDN will combine multiple concurrent cache fill requests into a small number of requests
to the origin.</rdfs:comment>
    <rdfs:domain rdf:resource="http://example.org/onto/class/google_compute_backend_service"/>
    <rdfs:range rdf:resource="http://www.w3.org/2001/XMLSchema#string"/>
  </owl:DatatypeProperty>
  <owl:DatatypeProperty rdf:about="http://example.org/onto/prop/google_compute_backend_service_serve_while_stale">
    <rdfs:label>serve_while_stale</rdfs:label>
    <rdfs:comment>Serve existing content from the cache (if available) when revalidating content with the origin, or when an error is encountered when refreshing the cache.</rdfs:comment>
    <rdfs:domain rdf:resource="http://example.org/onto/class/google_compute_backend_service"/>
    <rdfs:range rdf:resource="http://www.w3.org/2001/XMLSchema#string"/>
  </owl:DatatypeProperty>
  <owl:DatatypeProperty rdf:about="http://example.org/onto/prop/google_compute_backend_service_signed_url_cache_max_age_sec">
    <rdfs:label>signed_url_cache_max_age_sec</rdfs:label>
    <rdfs:comment>Maximum number of seconds the response to a signed URL request
will be considered fresh, defaults to 1hr (3600s). After this
time period, the response will be revalidated before
being served.

When serving responses to signed URL requests, Cloud CDN will
internally behave as though all responses from this backend had a
"Cache-Control: public, max-age=[TTL]" header, regardless of any
existing Cache-Control header. The actual headers served in
responses will not be altered.</rdfs:comment>
    <rdfs:domain rdf:resource="http://example.org/onto/class/google_compute_backend_service"/>
    <rdfs:range rdf:resource="http://www.w3.org/2001/XMLSchema#string"/>
  </owl:DatatypeProperty>
  <owl:DatatypeProperty rdf:about="http://example.org/onto/prop/google_compute_backend_service_header_name">
    <rdfs:label>header_name</rdfs:label>
    <rdfs:comment>The header field name to match on when bypassing cache. Values are case-insensitive.</rdfs:comment>
    <rdfs:domain rdf:resource="http://example.org/onto/class/google_compute_backend_service"/>
    <rdfs:range rdf:resource="http://www.w3.org/2001/XMLSchema#string"/>
  </owl:DatatypeProperty>
  <owl:DatatypeProperty rdf:about="http://example.org/onto/prop/google_compute_backend_service_include_host">
    <rdfs:label>include_host</rdfs:label>
    <rdfs:comment>If true requests to different hosts will be cached separately.</rdfs:comment>
    <rdfs:domain rdf:resource="http://example.org/onto/class/google_compute_backend_service"/>
    <rdfs:range rdf:resource="http://www.w3.org/2001/XMLSchema#string"/>
  </owl:DatatypeProperty>
  <owl:DatatypeProperty rdf:about="http://example.org/onto/prop/google_compute_backend_service_include_http_headers">
    <rdfs:label>include_http_headers</rdfs:label>
    <rdfs:comment>Allows HTTP request headers (by name) to be used in the
cache key.</rdfs:comment>
    <rdfs:domain rdf:resource="http://example.org/onto/class/google_compute_backend_service"/>
    <rdfs:range rdf:resource="http://www.w3.org/2001/XMLSchema#string"/>
  </owl:DatatypeProperty>
  <owl:DatatypeProperty rdf:about="http://example.org/onto/prop/google_compute_backend_service_include_named_cookies">
    <rdfs:label>include_named_cookies</rdfs:label>
    <rdfs:comment>Names of cookies to include in cache keys.</rdfs:comment>
    <rdfs:domain rdf:resource="http://example.org/onto/class/google_compute_backend_service"/>
    <rdfs:range rdf:resource="http://www.w3.org/2001/XMLSchema#string"/>
  </owl:DatatypeProperty>
  <owl:DatatypeProperty rdf:about="http://example.org/onto/prop/google_compute_backend_service_include_protocol">
    <rdfs:label>include_protocol</rdfs:label>
    <rdfs:comment>If true, http and https requests will be cached separately.</rdfs:comment>
    <rdfs:domain rdf:resource="http://example.org/onto/class/google_compute_backend_service"/>
    <rdfs:range rdf:resource="http://www.w3.org/2001/XMLSchema#string"/>
  </owl:DatatypeProperty>
  <owl:DatatypeProperty rdf:about="http://example.org/onto/prop/google_compute_backend_service_include_query_string">
    <rdfs:label>include_query_string</rdfs:label>
    <rdfs:comment>If true, include query string parameters in the cache key
according to query_string_whitelist and
query_string_blacklist. If neither is set, the entire query
string will be included.

If false, the query string will be excluded from the cache
key entirely.</rdfs:comment>
    <rdfs:domain rdf:resource="http://example.org/onto/class/google_compute_backend_service"/>
    <rdfs:range rdf:resource="http://www.w3.org/2001/XMLSchema#string"/>
  </owl:DatatypeProperty>
  <owl:DatatypeProperty rdf:about="http://example.org/onto/prop/google_compute_backend_service_query_string_blacklist">
    <rdfs:label>query_string_blacklist</rdfs:label>
    <rdfs:comment>Names of query string parameters to exclude in cache keys.

All other parameters will be included. Either specify
query_string_whitelist or query_string_blacklist, not both.
'&' and '=' will be percent encoded and not treated as
delimiters.</rdfs:comment>
    <rdfs:domain rdf:resource="http://example.org/onto/class/google_compute_backend_service"/>
    <rdfs:range rdf:resource="http://www.w3.org/2001/XMLSchema#string"/>
  </owl:DatatypeProperty>
  <owl:DatatypeProperty rdf:about="http://example.org/onto/prop/google_compute_backend_service_query_string_whitelist">
    <rdfs:label>query_string_whitelist</rdfs:label>
    <rdfs:comment>Names of query string parameters to include in cache keys.

All other parameters will be excluded. Either specify
query_string_whitelist or query_string_blacklist, not both.
'&' and '=' will be percent encoded and not treated as
delimiters.</rdfs:comment>
    <rdfs:domain rdf:resource="http://example.org/onto/class/google_compute_backend_service"/>
    <rdfs:range rdf:resource="http://www.w3.org/2001/XMLSchema#string"/>
  </owl:DatatypeProperty>
  <owl:DatatypeProperty rdf:about="http://example.org/onto/prop/google_compute_backend_service_code">
    <rdfs:label>code</rdfs:label>
    <rdfs:comment>The HTTP status code to define a TTL against. Only HTTP status codes 300, 301, 308, 404, 405, 410, 421, 451 and 501
can be specified as values, and you cannot specify a status code more than once.</rdfs:comment>
    <rdfs:domain rdf:resource="http://example.org/onto/class/google_compute_backend_service"/>
    <rdfs:range rdf:resource="http://www.w3.org/2001/XMLSchema#string"/>
  </owl:DatatypeProperty>
  <owl:DatatypeProperty rdf:about="http://example.org/onto/prop/google_compute_backend_service_ttl">
    <rdfs:label>ttl</rdfs:label>
    <rdfs:comment>The TTL (in seconds) for which to cache responses with the corresponding status code. The maximum allowed value is 1800s
(30 minutes), noting that infrequently accessed objects may be evicted from the cache before the defined TTL.</rdfs:comment>
    <rdfs:domain rdf:resource="http://example.org/onto/class/google_compute_backend_service"/>
    <rdfs:range rdf:resource="http://www.w3.org/2001/XMLSchema#string"/>
  </owl:DatatypeProperty>
  <owl:DatatypeProperty rdf:about="http://example.org/onto/prop/google_compute_backend_service_max_connections">
    <rdfs:label>max_connections</rdfs:label>
    <rdfs:comment>The maximum number of connections to the backend cluster.
Defaults to 1024.</rdfs:comment>
    <rdfs:domain rdf:resource="http://example.org/onto/class/google_compute_backend_service"/>
    <rdfs:range rdf:resource="http://www.w3.org/2001/XMLSchema#string"/>
  </owl:DatatypeProperty>
  <owl:DatatypeProperty rdf:about="http://example.org/onto/prop/google_compute_backend_service_max_pending_requests">
    <rdfs:label>max_pending_requests</rdfs:label>
    <rdfs:comment>The maximum number of pending requests to the backend cluster.
Defaults to 1024.</rdfs:comment>
    <rdfs:domain rdf:resource="http://example.org/onto/class/google_compute_backend_service"/>
    <rdfs:range rdf:resource="http://www.w3.org/2001/XMLSchema#string"/>
  </owl:DatatypeProperty>
  <owl:DatatypeProperty rdf:about="http://example.org/onto/prop/google_compute_backend_service_max_requests">
    <rdfs:label>max_requests</rdfs:label>
    <rdfs:comment>The maximum number of parallel requests to the backend cluster.
Defaults to 1024.</rdfs:comment>
    <rdfs:domain rdf:resource="http://example.org/onto/class/google_compute_backend_service"/>
    <rdfs:range rdf:resource="http://www.w3.org/2001/XMLSchema#string"/>
  </owl:DatatypeProperty>
  <owl:DatatypeProperty rdf:about="http://example.org/onto/prop/google_compute_backend_service_max_requests_per_connection">
    <rdfs:label>max_requests_per_connection</rdfs:label>
    <rdfs:comment>Maximum requests for a single backend connection. This parameter
is respected by both the HTTP/1.1 and HTTP/2 implementations. If
not specified, there is no limit. Setting this parameter to 1
will effectively disable keep alive.</rdfs:comment>
    <rdfs:domain rdf:resource="http://example.org/onto/class/google_compute_backend_service"/>
    <rdfs:range rdf:resource="http://www.w3.org/2001/XMLSchema#string"/>
  </owl:DatatypeProperty>
  <owl:DatatypeProperty rdf:about="http://example.org/onto/prop/google_compute_backend_service_max_retries">
    <rdfs:label>max_retries</rdfs:label>
    <rdfs:comment>The maximum number of parallel retries to the backend cluster.
Defaults to 3.</rdfs:comment>
    <rdfs:domain rdf:resource="http://example.org/onto/class/google_compute_backend_service"/>
    <rdfs:range rdf:resource="http://www.w3.org/2001/XMLSchema#string"/>
  </owl:DatatypeProperty>
  <owl:DatatypeProperty rdf:about="http://example.org/onto/prop/google_compute_backend_service_http_header_name">
    <rdfs:label>http_header_name</rdfs:label>
    <rdfs:comment>The hash based on the value of the specified header field.
This field is applicable if the sessionAffinity is set to HEADER_FIELD.</rdfs:comment>
    <rdfs:domain rdf:resource="http://example.org/onto/class/google_compute_backend_service"/>
    <rdfs:range rdf:resource="http://www.w3.org/2001/XMLSchema#string"/>
  </owl:DatatypeProperty>
  <owl:DatatypeProperty rdf:about="http://example.org/onto/prop/google_compute_backend_service_minimum_ring_size">
    <rdfs:label>minimum_ring_size</rdfs:label>
    <rdfs:comment>The minimum number of virtual nodes to use for the hash ring.
Larger ring sizes result in more granular load
distributions. If the number of hosts in the load balancing pool
is larger than the ring size, each host will be assigned a single
virtual node.
Defaults to 1024.</rdfs:comment>
    <rdfs:domain rdf:resource="http://example.org/onto/class/google_compute_backend_service"/>
    <rdfs:range rdf:resource="http://www.w3.org/2001/XMLSchema#string"/>
  </owl:DatatypeProperty>
  <owl:DatatypeProperty rdf:about="http://example.org/onto/prop/google_compute_backend_service_name">
    <rdfs:label>name</rdfs:label>
    <rdfs:comment>Name of the cookie.</rdfs:comment>
    <rdfs:domain rdf:resource="http://example.org/onto/class/google_compute_backend_service"/>
    <rdfs:range rdf:resource="http://www.w3.org/2001/XMLSchema#string"/>
  </owl:DatatypeProperty>
  <owl:DatatypeProperty rdf:about="http://example.org/onto/prop/google_compute_backend_service_path">
    <rdfs:label>path</rdfs:label>
    <rdfs:comment>Path to set for the cookie.</rdfs:comment>
    <rdfs:domain rdf:resource="http://example.org/onto/class/google_compute_backend_service"/>
    <rdfs:range rdf:resource="http://www.w3.org/2001/XMLSchema#string"/>
  </owl:DatatypeProperty>
  <owl:DatatypeProperty rdf:about="http://example.org/onto/prop/google_compute_backend_service_nanos">
    <rdfs:label>nanos</rdfs:label>
    <rdfs:comment>Span of time that's a fraction of a second at nanosecond
resolution. Durations less than one second are represented
with a 0 seconds field and a positive nanos field. Must
be from 0 to 999,999,999 inclusive.</rdfs:comment>
    <rdfs:domain rdf:resource="http://example.org/onto/class/google_compute_backend_service"/>
    <rdfs:range rdf:resource="http://www.w3.org/2001/XMLSchema#string"/>
  </owl:DatatypeProperty>
  <owl:DatatypeProperty rdf:about="http://example.org/onto/prop/google_compute_backend_service_seconds">
    <rdfs:label>seconds</rdfs:label>
    <rdfs:comment>Span of time at a resolution of a second.
Must be from 0 to 315,576,000,000 inclusive.</rdfs:comment>
    <rdfs:domain rdf:resource="http://example.org/onto/class/google_compute_backend_service"/>
    <rdfs:range rdf:resource="http://www.w3.org/2001/XMLSchema#string"/>
  </owl:DatatypeProperty>
  <owl:DatatypeProperty rdf:about="http://example.org/onto/prop/google_compute_backend_service_dry_run">
    <rdfs:label>dry_run</rdfs:label>
    <rdfs:comment>If true, the metric data is not used for load balancing.</rdfs:comment>
    <rdfs:domain rdf:resource="http://example.org/onto/class/google_compute_backend_service"/>
    <rdfs:range rdf:resource="http://www.w3.org/2001/XMLSchema#string"/>
  </owl:DatatypeProperty>
  <owl:DatatypeProperty rdf:about="http://example.org/onto/prop/google_compute_backend_service_name">
    <rdfs:label>name</rdfs:label>
    <rdfs:comment>Name of a custom utilization signal. The name must be 1-64 characters
long and match the regular expression [a-z]([-_.a-z0-9]*[a-z0-9])? which
means the first character must be a lowercase letter, and all following
characters must be a dash, period, underscore, lowercase letter, or
digit, except the last character, which cannot be a dash, period, or
underscore. For usage guidelines, see Custom Metrics balancing mode. This
field can only be used for a global or regional backend service with the
loadBalancingScheme set to <code>EXTERNAL_MANAGED</code>,
<code>INTERNAL_MANAGED</code> <code>INTERNAL_SELF_MANAGED</code>.</rdfs:comment>
    <rdfs:domain rdf:resource="http://example.org/onto/class/google_compute_backend_service"/>
    <rdfs:range rdf:resource="http://www.w3.org/2001/XMLSchema#string"/>
  </owl:DatatypeProperty>
  <owl:DatatypeProperty rdf:about="http://example.org/onto/prop/google_compute_backend_service_enabled">
    <rdfs:label>enabled</rdfs:label>
    <rdfs:comment>Whether the serving infrastructure will authenticate and authorize all incoming requests.</rdfs:comment>
    <rdfs:domain rdf:resource="http://example.org/onto/class/google_compute_backend_service"/>
    <rdfs:range rdf:resource="http://www.w3.org/2001/XMLSchema#string"/>
  </owl:DatatypeProperty>
  <owl:DatatypeProperty rdf:about="http://example.org/onto/prop/google_compute_backend_service_oauth2_client_id">
    <rdfs:label>oauth2_client_id</rdfs:label>
    <rdfs:comment>OAuth2 Client ID for IAP</rdfs:comment>
    <rdfs:domain rdf:resource="http://example.org/onto/class/google_compute_backend_service"/>
    <rdfs:range rdf:resource="http://www.w3.org/2001/XMLSchema#string"/>
  </owl:DatatypeProperty>
  <owl:DatatypeProperty rdf:about="http://example.org/onto/prop/google_compute_backend_service_oauth2_client_secret">
    <rdfs:label>oauth2_client_secret</rdfs:label>
    <rdfs:comment>OAuth2 Client Secret for IAP</rdfs:comment>
    <rdfs:domain rdf:resource="http://example.org/onto/class/google_compute_backend_service"/>
    <rdfs:range rdf:resource="http://www.w3.org/2001/XMLSchema#string"/>
  </owl:DatatypeProperty>
  <owl:DatatypeProperty rdf:about="http://example.org/onto/prop/google_compute_backend_service_oauth2_client_secret_sha256">
    <rdfs:label>oauth2_client_secret_sha256</rdfs:label>
    <rdfs:comment>OAuth2 Client Secret SHA-256 for IAP</rdfs:comment>
    <rdfs:domain rdf:resource="http://example.org/onto/class/google_compute_backend_service"/>
    <rdfs:range rdf:resource="http://www.w3.org/2001/XMLSchema#string"/>
  </owl:DatatypeProperty>
  <owl:DatatypeProperty rdf:about="http://example.org/onto/prop/google_compute_backend_service_data">
    <rdfs:label>data</rdfs:label>
    <rdfs:comment>An optional, arbitrary JSON object with configuration data, understood
by a locally installed custom policy implementation.</rdfs:comment>
    <rdfs:domain rdf:resource="http://example.org/onto/class/google_compute_backend_service"/>
    <rdfs:range rdf:resource="http://www.w3.org/2001/XMLSchema#string"/>
  </owl:DatatypeProperty>
  <owl:DatatypeProperty rdf:about="http://example.org/onto/prop/google_compute_backend_service_name">
    <rdfs:label>name</rdfs:label>
    <rdfs:comment>Identifies the custom policy.

The value should match the type the custom implementation is registered
with on the gRPC clients. It should follow protocol buffer
message naming conventions and include the full path (e.g.
myorg.CustomLbPolicy). The maximum length is 256 characters.

Note that specifying the same custom policy more than once for a
backend is not a valid configuration and will be rejected.</rdfs:comment>
    <rdfs:domain rdf:resource="http://example.org/onto/class/google_compute_backend_service"/>
    <rdfs:range rdf:resource="http://www.w3.org/2001/XMLSchema#string"/>
  </owl:DatatypeProperty>
  <owl:DatatypeProperty rdf:about="http://example.org/onto/prop/google_compute_backend_service_name">
    <rdfs:label>name</rdfs:label>
    <rdfs:comment>The name of a locality load balancer policy to be used. The value
should be one of the predefined ones as supported by localityLbPolicy,
although at the moment only ROUND_ROBIN is supported.

This field should only be populated when the customPolicy field is not
used.

Note that specifying the same policy more than once for a backend is
not a valid configuration and will be rejected.

The possible values are:

* 'ROUND_ROBIN': This is a simple policy in which each healthy backend
                is selected in round robin order.

* 'LEAST_REQUEST': An O(1) algorithm which selects two random healthy
                  hosts and picks the host which has fewer active requests.

* 'RING_HASH': The ring/modulo hash load balancer implements consistent
              hashing to backends. The algorithm has the property that the
              addition/removal of a host from a set of N hosts only affects
              1/N of the requests.

* 'RANDOM': The load balancer selects a random healthy host.

* 'ORIGINAL_DESTINATION': Backend host is selected based on the client
                          connection metadata, i.e., connections are opened
                          to the same address as the destination address of
                          the incoming connection before the connection
                          was redirected to the load balancer.

* 'MAGLEV': used as a drop in replacement for the ring hash load balancer.
            Maglev is not as stable as ring hash but has faster table lookup
            build times and host selection times. For more information about
            Maglev, refer to https://ai.google/research/pubs/pub44824 Possible values: ["ROUND_ROBIN", "LEAST_REQUEST", "RING_HASH", "RANDOM", "ORIGINAL_DESTINATION", "MAGLEV"]</rdfs:comment>
    <rdfs:domain rdf:resource="http://example.org/onto/class/google_compute_backend_service"/>
    <rdfs:range rdf:resource="http://www.w3.org/2001/XMLSchema#string"/>
  </owl:DatatypeProperty>
  <owl:DatatypeProperty rdf:about="http://example.org/onto/prop/google_compute_backend_service_enable">
    <rdfs:label>enable</rdfs:label>
    <rdfs:comment>Whether to enable logging for the load balancer traffic served by this backend service.</rdfs:comment>
    <rdfs:domain rdf:resource="http://example.org/onto/class/google_compute_backend_service"/>
    <rdfs:range rdf:resource="http://www.w3.org/2001/XMLSchema#string"/>
  </owl:DatatypeProperty>
  <owl:DatatypeProperty rdf:about="http://example.org/onto/prop/google_compute_backend_service_optional_fields">
    <rdfs:label>optional_fields</rdfs:label>
    <rdfs:comment>This field can only be specified if logging is enabled for this backend service and "logConfig.optionalMode"
was set to CUSTOM. Contains a list of optional fields you want to include in the logs.
For example: serverInstance, serverGkeDetails.cluster, serverGkeDetails.pod.podNamespace
For example: orca_load_report, tls.protocol</rdfs:comment>
    <rdfs:domain rdf:resource="http://example.org/onto/class/google_compute_backend_service"/>
    <rdfs:range rdf:resource="http://www.w3.org/2001/XMLSchema#string"/>
  </owl:DatatypeProperty>
  <owl:DatatypeProperty rdf:about="http://example.org/onto/prop/google_compute_backend_service_optional_mode">
    <rdfs:label>optional_mode</rdfs:label>
    <rdfs:comment>Specifies the optional logging mode for the load balancer traffic.
Supported values: INCLUDE_ALL_OPTIONAL, EXCLUDE_ALL_OPTIONAL, CUSTOM. Possible values: ["INCLUDE_ALL_OPTIONAL", "EXCLUDE_ALL_OPTIONAL", "CUSTOM"]</rdfs:comment>
    <rdfs:domain rdf:resource="http://example.org/onto/class/google_compute_backend_service"/>
    <rdfs:range rdf:resource="http://www.w3.org/2001/XMLSchema#string"/>
  </owl:DatatypeProperty>
  <owl:DatatypeProperty rdf:about="http://example.org/onto/prop/google_compute_backend_service_sample_rate">
    <rdfs:label>sample_rate</rdfs:label>
    <rdfs:comment>This field can only be specified if logging is enabled for this backend service. The value of
the field must be in [0, 1]. This configures the sampling rate of requests to the load balancer
where 1.0 means all logged requests are reported and 0.0 means no logged requests are reported.
The default value is 1.0.</rdfs:comment>
    <rdfs:domain rdf:resource="http://example.org/onto/class/google_compute_backend_service"/>
    <rdfs:range rdf:resource="http://www.w3.org/2001/XMLSchema#string"/>
  </owl:DatatypeProperty>
  <owl:DatatypeProperty rdf:about="http://example.org/onto/prop/google_compute_backend_service_nanos">
    <rdfs:label>nanos</rdfs:label>
    <rdfs:comment>Span of time that's a fraction of a second at nanosecond resolution.
Durations less than one second are represented with a 0 seconds field and a positive nanos field.
Must be from 0 to 999,999,999 inclusive.</rdfs:comment>
    <rdfs:domain rdf:resource="http://example.org/onto/class/google_compute_backend_service"/>
    <rdfs:range rdf:resource="http://www.w3.org/2001/XMLSchema#string"/>
  </owl:DatatypeProperty>
  <owl:DatatypeProperty rdf:about="http://example.org/onto/prop/google_compute_backend_service_seconds">
    <rdfs:label>seconds</rdfs:label>
    <rdfs:comment>Span of time at a resolution of a second. Must be from 0 to 315,576,000,000 inclusive. (int64 format)</rdfs:comment>
    <rdfs:domain rdf:resource="http://example.org/onto/class/google_compute_backend_service"/>
    <rdfs:range rdf:resource="http://www.w3.org/2001/XMLSchema#string"/>
  </owl:DatatypeProperty>
  <owl:DatatypeProperty rdf:about="http://example.org/onto/prop/google_compute_backend_service_consecutive_errors">
    <rdfs:label>consecutive_errors</rdfs:label>
    <rdfs:comment>Number of errors before a host is ejected from the connection pool. When the
backend host is accessed over HTTP, a 5xx return code qualifies as an error.
Defaults to 5.</rdfs:comment>
    <rdfs:domain rdf:resource="http://example.org/onto/class/google_compute_backend_service"/>
    <rdfs:range rdf:resource="http://www.w3.org/2001/XMLSchema#string"/>
  </owl:DatatypeProperty>
  <owl:DatatypeProperty rdf:about="http://example.org/onto/prop/google_compute_backend_service_consecutive_gateway_failure">
    <rdfs:label>consecutive_gateway_failure</rdfs:label>
    <rdfs:comment>The number of consecutive gateway failures (502, 503, 504 status or connection
errors that are mapped to one of those status codes) before a consecutive
gateway failure ejection occurs. Defaults to 5.</rdfs:comment>
    <rdfs:domain rdf:resource="http://example.org/onto/class/google_compute_backend_service"/>
    <rdfs:range rdf:resource="http://www.w3.org/2001/XMLSchema#string"/>
  </owl:DatatypeProperty>
  <owl:DatatypeProperty rdf:about="http://example.org/onto/prop/google_compute_backend_service_enforcing_consecutive_errors">
    <rdfs:label>enforcing_consecutive_errors</rdfs:label>
    <rdfs:comment>The percentage chance that a host will be actually ejected when an outlier
status is detected through consecutive 5xx. This setting can be used to disable
ejection or to ramp it up slowly. Defaults to 100.</rdfs:comment>
    <rdfs:domain rdf:resource="http://example.org/onto/class/google_compute_backend_service"/>
    <rdfs:range rdf:resource="http://www.w3.org/2001/XMLSchema#string"/>
  </owl:DatatypeProperty>
  <owl:DatatypeProperty rdf:about="http://example.org/onto/prop/google_compute_backend_service_enforcing_consecutive_gateway_failure">
    <rdfs:label>enforcing_consecutive_gateway_failure</rdfs:label>
    <rdfs:comment>The percentage chance that a host will be actually ejected when an outlier
status is detected through consecutive gateway failures. This setting can be
used to disable ejection or to ramp it up slowly. Defaults to 0.</rdfs:comment>
    <rdfs:domain rdf:resource="http://example.org/onto/class/google_compute_backend_service"/>
    <rdfs:range rdf:resource="http://www.w3.org/2001/XMLSchema#string"/>
  </owl:DatatypeProperty>
  <owl:DatatypeProperty rdf:about="http://example.org/onto/prop/google_compute_backend_service_enforcing_success_rate">
    <rdfs:label>enforcing_success_rate</rdfs:label>
    <rdfs:comment>The percentage chance that a host will be actually ejected when an outlier
status is detected through success rate statistics. This setting can be used to
disable ejection or to ramp it up slowly. Defaults to 100.</rdfs:comment>
    <rdfs:domain rdf:resource="http://example.org/onto/class/google_compute_backend_service"/>
    <rdfs:range rdf:resource="http://www.w3.org/2001/XMLSchema#string"/>
  </owl:DatatypeProperty>
  <owl:DatatypeProperty rdf:about="http://example.org/onto/prop/google_compute_backend_service_max_ejection_percent">
    <rdfs:label>max_ejection_percent</rdfs:label>
    <rdfs:comment>Maximum percentage of hosts in the load balancing pool for the backend service
that can be ejected. Defaults to 10%.</rdfs:comment>
    <rdfs:domain rdf:resource="http://example.org/onto/class/google_compute_backend_service"/>
    <rdfs:range rdf:resource="http://www.w3.org/2001/XMLSchema#string"/>
  </owl:DatatypeProperty>
  <owl:DatatypeProperty rdf:about="http://example.org/onto/prop/google_compute_backend_service_success_rate_minimum_hosts">
    <rdfs:label>success_rate_minimum_hosts</rdfs:label>
    <rdfs:comment>The number of hosts in a cluster that must have enough request volume to detect
success rate outliers. If the number of hosts is less than this setting, outlier
detection via success rate statistics is not performed for any host in the
cluster. Defaults to 5.</rdfs:comment>
    <rdfs:domain rdf:resource="http://example.org/onto/class/google_compute_backend_service"/>
    <rdfs:range rdf:resource="http://www.w3.org/2001/XMLSchema#string"/>
  </owl:DatatypeProperty>
  <owl:DatatypeProperty rdf:about="http://example.org/onto/prop/google_compute_backend_service_success_rate_request_volume">
    <rdfs:label>success_rate_request_volume</rdfs:label>
    <rdfs:comment>The minimum number of total requests that must be collected in one interval (as
defined by the interval duration above) to include this host in success rate
based outlier detection. If the volume is lower than this setting, outlier
detection via success rate statistics is not performed for that host. Defaults
to 100.</rdfs:comment>
    <rdfs:domain rdf:resource="http://example.org/onto/class/google_compute_backend_service"/>
    <rdfs:range rdf:resource="http://www.w3.org/2001/XMLSchema#string"/>
  </owl:DatatypeProperty>
  <owl:DatatypeProperty rdf:about="http://example.org/onto/prop/google_compute_backend_service_success_rate_stdev_factor">
    <rdfs:label>success_rate_stdev_factor</rdfs:label>
    <rdfs:comment>This factor is used to determine the ejection threshold for success rate outlier
ejection. The ejection threshold is the difference between the mean success
rate, and the product of this factor and the standard deviation of the mean
success rate: mean - (stdev * success_rate_stdev_factor). This factor is divided
by a thousand to get a double. That is, if the desired factor is 1.9, the
runtime value should be 1900. Defaults to 1900.</rdfs:comment>
    <rdfs:domain rdf:resource="http://example.org/onto/class/google_compute_backend_service"/>
    <rdfs:range rdf:resource="http://www.w3.org/2001/XMLSchema#string"/>
  </owl:DatatypeProperty>
  <owl:DatatypeProperty rdf:about="http://example.org/onto/prop/google_compute_backend_service_nanos">
    <rdfs:label>nanos</rdfs:label>
    <rdfs:comment>Span of time that's a fraction of a second at nanosecond resolution. Durations
less than one second are represented with a 0 'seconds' field and a positive
'nanos' field. Must be from 0 to 999,999,999 inclusive.</rdfs:comment>
    <rdfs:domain rdf:resource="http://example.org/onto/class/google_compute_backend_service"/>
    <rdfs:range rdf:resource="http://www.w3.org/2001/XMLSchema#string"/>
  </owl:DatatypeProperty>
  <owl:DatatypeProperty rdf:about="http://example.org/onto/prop/google_compute_backend_service_seconds">
    <rdfs:label>seconds</rdfs:label>
    <rdfs:comment>Span of time at a resolution of a second. Must be from 0 to 315,576,000,000
inclusive.</rdfs:comment>
    <rdfs:domain rdf:resource="http://example.org/onto/class/google_compute_backend_service"/>
    <rdfs:range rdf:resource="http://www.w3.org/2001/XMLSchema#string"/>
  </owl:DatatypeProperty>
  <owl:DatatypeProperty rdf:about="http://example.org/onto/prop/google_compute_backend_service_nanos">
    <rdfs:label>nanos</rdfs:label>
    <rdfs:comment>Span of time that's a fraction of a second at nanosecond resolution. Durations
less than one second are represented with a 0 'seconds' field and a positive
'nanos' field. Must be from 0 to 999,999,999 inclusive.</rdfs:comment>
    <rdfs:domain rdf:resource="http://example.org/onto/class/google_compute_backend_service"/>
    <rdfs:range rdf:resource="http://www.w3.org/2001/XMLSchema#string"/>
  </owl:DatatypeProperty>
  <owl:DatatypeProperty rdf:about="http://example.org/onto/prop/google_compute_backend_service_seconds">
    <rdfs:label>seconds</rdfs:label>
    <rdfs:comment>Span of time at a resolution of a second. Must be from 0 to 315,576,000,000
inclusive.</rdfs:comment>
    <rdfs:domain rdf:resource="http://example.org/onto/class/google_compute_backend_service"/>
    <rdfs:range rdf:resource="http://www.w3.org/2001/XMLSchema#string"/>
  </owl:DatatypeProperty>
  <owl:DatatypeProperty rdf:about="http://example.org/onto/prop/google_compute_backend_service_resource_manager_tags">
    <rdfs:label>resource_manager_tags</rdfs:label>
    <rdfs:comment>Resource manager tags to be bound to the backend service. Tag keys and values have the
same definition as resource manager tags. Keys must be in the format tagKeys/{tag_key_id},
and values are in the format tagValues/456.</rdfs:comment>
    <rdfs:domain rdf:resource="http://example.org/onto/class/google_compute_backend_service"/>
    <rdfs:range rdf:resource="http://www.w3.org/2001/XMLSchema#string"/>
  </owl:DatatypeProperty>
  <owl:DatatypeProperty rdf:about="http://example.org/onto/prop/google_compute_backend_service_client_tls_policy">
    <rdfs:label>client_tls_policy</rdfs:label>
    <rdfs:comment>ClientTlsPolicy is a resource that specifies how a client should authenticate
connections to backends of a service. This resource itself does not affect
configuration unless it is attached to a backend service resource.</rdfs:comment>
    <rdfs:domain rdf:resource="http://example.org/onto/class/google_compute_backend_service"/>
    <rdfs:range rdf:resource="http://www.w3.org/2001/XMLSchema#string"/>
  </owl:DatatypeProperty>
  <owl:DatatypeProperty rdf:about="http://example.org/onto/prop/google_compute_backend_service_subject_alt_names">
    <rdfs:label>subject_alt_names</rdfs:label>
    <rdfs:comment>A list of alternate names to verify the subject identity in the certificate.
If specified, the client will verify that the server certificate's subject
alt name matches one of the specified values.</rdfs:comment>
    <rdfs:domain rdf:resource="http://example.org/onto/class/google_compute_backend_service"/>
    <rdfs:range rdf:resource="http://www.w3.org/2001/XMLSchema#string"/>
  </owl:DatatypeProperty>
  <owl:DatatypeProperty rdf:about="http://example.org/onto/prop/google_compute_backend_service_access_key">
    <rdfs:label>access_key</rdfs:label>
    <rdfs:comment>The access key used for s3 bucket authentication.
Required for updating or creating a backend that uses AWS v4 signature authentication, but will not be returned as part of the configuration when queried with a REST API GET request.</rdfs:comment>
    <rdfs:domain rdf:resource="http://example.org/onto/class/google_compute_backend_service"/>
    <rdfs:range rdf:resource="http://www.w3.org/2001/XMLSchema#string"/>
  </owl:DatatypeProperty>
  <owl:DatatypeProperty rdf:about="http://example.org/onto/prop/google_compute_backend_service_access_key_id">
    <rdfs:label>access_key_id</rdfs:label>
    <rdfs:comment>The identifier of an access key used for s3 bucket authentication.</rdfs:comment>
    <rdfs:domain rdf:resource="http://example.org/onto/class/google_compute_backend_service"/>
    <rdfs:range rdf:resource="http://www.w3.org/2001/XMLSchema#string"/>
  </owl:DatatypeProperty>
  <owl:DatatypeProperty rdf:about="http://example.org/onto/prop/google_compute_backend_service_access_key_version">
    <rdfs:label>access_key_version</rdfs:label>
    <rdfs:comment>The optional version identifier for the access key. You can use this to keep track of different iterations of your access key.</rdfs:comment>
    <rdfs:domain rdf:resource="http://example.org/onto/class/google_compute_backend_service"/>
    <rdfs:range rdf:resource="http://www.w3.org/2001/XMLSchema#string"/>
  </owl:DatatypeProperty>
  <owl:DatatypeProperty rdf:about="http://example.org/onto/prop/google_compute_backend_service_origin_region">
    <rdfs:label>origin_region</rdfs:label>
    <rdfs:comment>The name of the cloud region of your origin. This is a free-form field with the name of the region your cloud uses to host your origin.
For example, "us-east-1" for AWS or "us-ashburn-1" for OCI.</rdfs:comment>
    <rdfs:domain rdf:resource="http://example.org/onto/class/google_compute_backend_service"/>
    <rdfs:range rdf:resource="http://www.w3.org/2001/XMLSchema#string"/>
  </owl:DatatypeProperty>
  <owl:DatatypeProperty rdf:about="http://example.org/onto/prop/google_compute_backend_service_name">
    <rdfs:label>name</rdfs:label>
    <rdfs:comment>Name of the cookie.</rdfs:comment>
    <rdfs:domain rdf:resource="http://example.org/onto/class/google_compute_backend_service"/>
    <rdfs:range rdf:resource="http://www.w3.org/2001/XMLSchema#string"/>
  </owl:DatatypeProperty>
  <owl:DatatypeProperty rdf:about="http://example.org/onto/prop/google_compute_backend_service_path">
    <rdfs:label>path</rdfs:label>
    <rdfs:comment>Path to set for the cookie.</rdfs:comment>
    <rdfs:domain rdf:resource="http://example.org/onto/class/google_compute_backend_service"/>
    <rdfs:range rdf:resource="http://www.w3.org/2001/XMLSchema#string"/>
  </owl:DatatypeProperty>
  <owl:DatatypeProperty rdf:about="http://example.org/onto/prop/google_compute_backend_service_nanos">
    <rdfs:label>nanos</rdfs:label>
    <rdfs:comment>Span of time that's a fraction of a second at nanosecond
resolution. Durations less than one second are represented
with a 0 seconds field and a positive nanos field. Must
be from 0 to 999,999,999 inclusive.</rdfs:comment>
    <rdfs:domain rdf:resource="http://example.org/onto/class/google_compute_backend_service"/>
    <rdfs:range rdf:resource="http://www.w3.org/2001/XMLSchema#string"/>
  </owl:DatatypeProperty>
  <owl:DatatypeProperty rdf:about="http://example.org/onto/prop/google_compute_backend_service_seconds">
    <rdfs:label>seconds</rdfs:label>
    <rdfs:comment>Span of time at a resolution of a second.
Must be from 0 to 315,576,000,000 inclusive.</rdfs:comment>
    <rdfs:domain rdf:resource="http://example.org/onto/class/google_compute_backend_service"/>
    <rdfs:range rdf:resource="http://www.w3.org/2001/XMLSchema#string"/>
  </owl:DatatypeProperty>
  <owl:DatatypeProperty rdf:about="http://example.org/onto/prop/google_compute_backend_service_create">
    <rdfs:label>create</rdfs:label>
    <rdfs:domain rdf:resource="http://example.org/onto/class/google_compute_backend_service"/>
    <rdfs:range rdf:resource="http://www.w3.org/2001/XMLSchema#string"/>
  </owl:DatatypeProperty>
  <owl:DatatypeProperty rdf:about="http://example.org/onto/prop/google_compute_backend_service_delete">
    <rdfs:label>delete</rdfs:label>
    <rdfs:domain rdf:resource="http://example.org/onto/class/google_compute_backend_service"/>
    <rdfs:range rdf:resource="http://www.w3.org/2001/XMLSchema#string"/>
  </owl:DatatypeProperty>
  <owl:DatatypeProperty rdf:about="http://example.org/onto/prop/google_compute_backend_service_update">
    <rdfs:label>update</rdfs:label>
    <rdfs:domain rdf:resource="http://example.org/onto/class/google_compute_backend_service"/>
    <rdfs:range rdf:resource="http://www.w3.org/2001/XMLSchema#string"/>
  </owl:DatatypeProperty>
  <owl:DatatypeProperty rdf:about="http://example.org/onto/prop/google_compute_backend_service_authentication_config">
    <rdfs:label>authentication_config</rdfs:label>
    <rdfs:comment>Reference to the BackendAuthenticationConfig resource from the networksecurity.googleapis.com namespace.
Can be used in authenticating TLS connections to the backend, as specified by the authenticationMode field.
Can only be specified if authenticationMode is not NONE.</rdfs:comment>
    <rdfs:domain rdf:resource="http://example.org/onto/class/google_compute_backend_service"/>
    <rdfs:range rdf:resource="http://www.w3.org/2001/XMLSchema#string"/>
  </owl:DatatypeProperty>
  <owl:DatatypeProperty rdf:about="http://example.org/onto/prop/google_compute_backend_service_sni">
    <rdfs:label>sni</rdfs:label>
    <rdfs:comment>Server Name Indication - see RFC3546 section 3.1. If set, the load balancer sends this string as the SNI hostname in the
TLS connection to the backend, and requires that this string match a Subject Alternative Name (SAN) in the backend's
server certificate. With a Regional Internet NEG backend, if the SNI is specified here, the load balancer uses it
regardless of whether the Regional Internet NEG is specified with FQDN or IP address and port.</rdfs:comment>
    <rdfs:domain rdf:resource="http://example.org/onto/class/google_compute_backend_service"/>
    <rdfs:range rdf:resource="http://www.w3.org/2001/XMLSchema#string"/>
  </owl:DatatypeProperty>
  <owl:DatatypeProperty rdf:about="http://example.org/onto/prop/google_compute_backend_service_dns_name">
    <rdfs:label>dns_name</rdfs:label>
    <rdfs:comment>The SAN specified as a DNS Name.</rdfs:comment>
    <rdfs:domain rdf:resource="http://example.org/onto/class/google_compute_backend_service"/>
    <rdfs:range rdf:resource="http://www.w3.org/2001/XMLSchema#string"/>
  </owl:DatatypeProperty>
  <owl:DatatypeProperty rdf:about="http://example.org/onto/prop/google_compute_backend_service_uniform_resource_identifier">
    <rdfs:label>uniform_resource_identifier</rdfs:label>
    <rdfs:comment>The SAN specified as a URI.</rdfs:comment>
    <rdfs:domain rdf:resource="http://example.org/onto/class/google_compute_backend_service"/>
    <rdfs:range rdf:resource="http://www.w3.org/2001/XMLSchema#string"/>
  </owl:DatatypeProperty>
</rdf:RDF>
