<?xml version="1.0" encoding="UTF-8"?>
<rdf:RDF
  xmlns:rdf="http://www.w3.org/1999/02/22-rdf-syntax-ns#"
  xmlns:rdfs="http://www.w3.org/2000/01/rdf-schema#"
  xmlns:owl="http://www.w3.org/2002/07/owl#"
  xmlns:xsd="http://www.w3.org/2001/XMLSchema#"
  xml:base="http://example.org/onto/">
  <owl:Class rdf:about="http://example.org/onto/class/google_compute_per_instance_config">
    <rdfs:label>google_compute_per_instance_config</rdfs:label>
    <rdfs:comment>#
#     ***     AUTO GENERATED CODE    ***    Type: MMv1     ***
#
# ----------------------------------------------------------------------------
#
#     This code is generated by Magic Modules using the following:
#
#     Configuration: https:#github.com/GoogleCloudPlatform/magic-modules/tree/main/mmv1/products/compute/PerInstanceConfig.yaml
#     Template:      https:#github.com/GoogleCloudPlatform/magic-modules/tree/main/mmv1/templates/terraform/resource.html.markdown.tmpl
#
#     DO NOT EDIT this file directly. Any changes made to this file will be
#     overwritten during the next generation cycle.
#
# ----------------------------------------------------------------------------
subcategory: "Compute Engine"
description: |-
  A config defined for a single managed instance that belongs to an instance group manager.
---</rdfs:comment>
  </owl:Class>
  <owl:DatatypeProperty rdf:about="http://example.org/onto/prop/google_compute_per_instance_config_id">
    <rdfs:label>id</rdfs:label>
    <rdfs:domain rdf:resource="http://example.org/onto/class/google_compute_per_instance_config"/>
    <rdfs:range rdf:resource="http://www.w3.org/2001/XMLSchema#string"/>
  </owl:DatatypeProperty>
  <owl:DatatypeProperty rdf:about="http://example.org/onto/prop/google_compute_per_instance_config_instance_group_manager">
    <rdfs:label>instance_group_manager</rdfs:label>
    <rdfs:comment>The instance group manager this instance config is part of.</rdfs:comment>
    <rdfs:domain rdf:resource="http://example.org/onto/class/google_compute_per_instance_config"/>
    <rdfs:range rdf:resource="http://www.w3.org/2001/XMLSchema#string"/>
  </owl:DatatypeProperty>
  <owl:DatatypeProperty rdf:about="http://example.org/onto/prop/google_compute_per_instance_config_minimal_action">
    <rdfs:label>minimal_action</rdfs:label>
    <rdfs:comment>The minimal action to perform on the instance during an update.
Default is 'NONE'. Possible values are:
* REPLACE
* RESTART
* REFRESH
* NONE</rdfs:comment>
    <rdfs:domain rdf:resource="http://example.org/onto/class/google_compute_per_instance_config"/>
    <rdfs:range rdf:resource="http://www.w3.org/2001/XMLSchema#string"/>
  </owl:DatatypeProperty>
  <owl:DatatypeProperty rdf:about="http://example.org/onto/prop/google_compute_per_instance_config_most_disruptive_allowed_action">
    <rdfs:label>most_disruptive_allowed_action</rdfs:label>
    <rdfs:comment>The most disruptive action to perform on the instance during an update.
Default is 'REPLACE'. Possible values are:
* REPLACE
* RESTART
* REFRESH
* NONE</rdfs:comment>
    <rdfs:domain rdf:resource="http://example.org/onto/class/google_compute_per_instance_config"/>
    <rdfs:range rdf:resource="http://www.w3.org/2001/XMLSchema#string"/>
  </owl:DatatypeProperty>
  <owl:DatatypeProperty rdf:about="http://example.org/onto/prop/google_compute_per_instance_config_name">
    <rdfs:label>name</rdfs:label>
    <rdfs:comment>The name for this per-instance config and its corresponding instance.</rdfs:comment>
    <rdfs:domain rdf:resource="http://example.org/onto/class/google_compute_per_instance_config"/>
    <rdfs:range rdf:resource="http://www.w3.org/2001/XMLSchema#string"/>
  </owl:DatatypeProperty>
  <owl:DatatypeProperty rdf:about="http://example.org/onto/prop/google_compute_per_instance_config_project">
    <rdfs:label>project</rdfs:label>
    <rdfs:domain rdf:resource="http://example.org/onto/class/google_compute_per_instance_config"/>
    <rdfs:range rdf:resource="http://www.w3.org/2001/XMLSchema#string"/>
  </owl:DatatypeProperty>
  <owl:DatatypeProperty rdf:about="http://example.org/onto/prop/google_compute_per_instance_config_remove_instance_on_destroy">
    <rdfs:label>remove_instance_on_destroy</rdfs:label>
    <rdfs:comment>When true, deleting this config will immediately remove the underlying instance.
When false, deleting this config will use the behavior as determined by remove_instance_on_destroy.</rdfs:comment>
    <rdfs:domain rdf:resource="http://example.org/onto/class/google_compute_per_instance_config"/>
    <rdfs:range rdf:resource="http://www.w3.org/2001/XMLSchema#string"/>
  </owl:DatatypeProperty>
  <owl:DatatypeProperty rdf:about="http://example.org/onto/prop/google_compute_per_instance_config_remove_instance_state_on_destroy">
    <rdfs:label>remove_instance_state_on_destroy</rdfs:label>
    <rdfs:comment>When true, deleting this config will immediately remove any specified state from the underlying instance.
When false, deleting this config will *not* immediately remove any state from the underlying instance.
State will be removed on the next instance recreation or update.</rdfs:comment>
    <rdfs:domain rdf:resource="http://example.org/onto/class/google_compute_per_instance_config"/>
    <rdfs:range rdf:resource="http://www.w3.org/2001/XMLSchema#string"/>
  </owl:DatatypeProperty>
  <owl:DatatypeProperty rdf:about="http://example.org/onto/prop/google_compute_per_instance_config_zone">
    <rdfs:label>zone</rdfs:label>
    <rdfs:comment>Zone where the containing instance group manager is located</rdfs:comment>
    <rdfs:domain rdf:resource="http://example.org/onto/class/google_compute_per_instance_config"/>
    <rdfs:range rdf:resource="http://www.w3.org/2001/XMLSchema#string"/>
  </owl:DatatypeProperty>
  <owl:DatatypeProperty rdf:about="http://example.org/onto/prop/google_compute_per_instance_config_metadata">
    <rdfs:label>metadata</rdfs:label>
    <rdfs:comment>Preserved metadata defined for this instance. This is a list of key->value pairs.</rdfs:comment>
    <rdfs:domain rdf:resource="http://example.org/onto/class/google_compute_per_instance_config"/>
    <rdfs:range rdf:resource="http://www.w3.org/2001/XMLSchema#string"/>
  </owl:DatatypeProperty>
  <owl:DatatypeProperty rdf:about="http://example.org/onto/prop/google_compute_per_instance_config_delete_rule">
    <rdfs:label>delete_rule</rdfs:label>
    <rdfs:comment>A value that prescribes what should happen to the stateful disk when the VM instance is deleted.
The available options are 'NEVER' and 'ON_PERMANENT_INSTANCE_DELETION'.
'NEVER' - detach the disk when the VM is deleted, but do not delete the disk.
'ON_PERMANENT_INSTANCE_DELETION' will delete the stateful disk when the VM is permanently
deleted from the instance group. Default value: "NEVER" Possible values: ["NEVER", "ON_PERMANENT_INSTANCE_DELETION"]</rdfs:comment>
    <rdfs:domain rdf:resource="http://example.org/onto/class/google_compute_per_instance_config"/>
    <rdfs:range rdf:resource="http://www.w3.org/2001/XMLSchema#string"/>
  </owl:DatatypeProperty>
  <owl:DatatypeProperty rdf:about="http://example.org/onto/prop/google_compute_per_instance_config_device_name">
    <rdfs:label>device_name</rdfs:label>
    <rdfs:comment>A unique device name that is reflected into the /dev/ tree of a Linux operating system running within the instance.</rdfs:comment>
    <rdfs:domain rdf:resource="http://example.org/onto/class/google_compute_per_instance_config"/>
    <rdfs:range rdf:resource="http://www.w3.org/2001/XMLSchema#string"/>
  </owl:DatatypeProperty>
  <owl:DatatypeProperty rdf:about="http://example.org/onto/prop/google_compute_per_instance_config_mode">
    <rdfs:label>mode</rdfs:label>
    <rdfs:comment>The mode of the disk. Default value: "READ_WRITE" Possible values: ["READ_ONLY", "READ_WRITE"]</rdfs:comment>
    <rdfs:domain rdf:resource="http://example.org/onto/class/google_compute_per_instance_config"/>
    <rdfs:range rdf:resource="http://www.w3.org/2001/XMLSchema#string"/>
  </owl:DatatypeProperty>
  <owl:DatatypeProperty rdf:about="http://example.org/onto/prop/google_compute_per_instance_config_source">
    <rdfs:label>source</rdfs:label>
    <rdfs:comment>The URI of an existing persistent disk to attach under the specified device-name in the format
'projects/project-id/zones/zone/disks/disk-name'.</rdfs:comment>
    <rdfs:domain rdf:resource="http://example.org/onto/class/google_compute_per_instance_config"/>
    <rdfs:range rdf:resource="http://www.w3.org/2001/XMLSchema#string"/>
  </owl:DatatypeProperty>
  <owl:DatatypeProperty rdf:about="http://example.org/onto/prop/google_compute_per_instance_config_auto_delete">
    <rdfs:label>auto_delete</rdfs:label>
    <rdfs:comment>These stateful IPs will never be released during autohealing, update or VM instance recreate operations. This flag is used to configure if the IP reservation should be deleted after it is no longer used by the group, e.g. when the given instance or the whole group is deleted. Default value: "NEVER" Possible values: ["NEVER", "ON_PERMANENT_INSTANCE_DELETION"]</rdfs:comment>
    <rdfs:domain rdf:resource="http://example.org/onto/class/google_compute_per_instance_config"/>
    <rdfs:range rdf:resource="http://www.w3.org/2001/XMLSchema#string"/>
  </owl:DatatypeProperty>
  <owl:DatatypeProperty rdf:about="http://example.org/onto/prop/google_compute_per_instance_config_interface_name">
    <rdfs:label>interface_name</rdfs:label>
    <rdfs:domain rdf:resource="http://example.org/onto/class/google_compute_per_instance_config"/>
    <rdfs:range rdf:resource="http://www.w3.org/2001/XMLSchema#string"/>
  </owl:DatatypeProperty>
  <owl:DatatypeProperty rdf:about="http://example.org/onto/prop/google_compute_per_instance_config_address">
    <rdfs:label>address</rdfs:label>
    <rdfs:comment>The URL of the reservation for this IP address.</rdfs:comment>
    <rdfs:domain rdf:resource="http://example.org/onto/class/google_compute_per_instance_config"/>
    <rdfs:range rdf:resource="http://www.w3.org/2001/XMLSchema#string"/>
  </owl:DatatypeProperty>
  <owl:DatatypeProperty rdf:about="http://example.org/onto/prop/google_compute_per_instance_config_auto_delete">
    <rdfs:label>auto_delete</rdfs:label>
    <rdfs:comment>These stateful IPs will never be released during autohealing, update or VM instance recreate operations. This flag is used to configure if the IP reservation should be deleted after it is no longer used by the group, e.g. when the given instance or the whole group is deleted. Default value: "NEVER" Possible values: ["NEVER", "ON_PERMANENT_INSTANCE_DELETION"]</rdfs:comment>
    <rdfs:domain rdf:resource="http://example.org/onto/class/google_compute_per_instance_config"/>
    <rdfs:range rdf:resource="http://www.w3.org/2001/XMLSchema#string"/>
  </owl:DatatypeProperty>
  <owl:DatatypeProperty rdf:about="http://example.org/onto/prop/google_compute_per_instance_config_interface_name">
    <rdfs:label>interface_name</rdfs:label>
    <rdfs:domain rdf:resource="http://example.org/onto/class/google_compute_per_instance_config"/>
    <rdfs:range rdf:resource="http://www.w3.org/2001/XMLSchema#string"/>
  </owl:DatatypeProperty>
  <owl:DatatypeProperty rdf:about="http://example.org/onto/prop/google_compute_per_instance_config_address">
    <rdfs:label>address</rdfs:label>
    <rdfs:comment>The URL of the reservation for this IP address.</rdfs:comment>
    <rdfs:domain rdf:resource="http://example.org/onto/class/google_compute_per_instance_config"/>
    <rdfs:range rdf:resource="http://www.w3.org/2001/XMLSchema#string"/>
  </owl:DatatypeProperty>
  <owl:DatatypeProperty rdf:about="http://example.org/onto/prop/google_compute_per_instance_config_create">
    <rdfs:label>create</rdfs:label>
    <rdfs:domain rdf:resource="http://example.org/onto/class/google_compute_per_instance_config"/>
    <rdfs:range rdf:resource="http://www.w3.org/2001/XMLSchema#string"/>
  </owl:DatatypeProperty>
  <owl:DatatypeProperty rdf:about="http://example.org/onto/prop/google_compute_per_instance_config_delete">
    <rdfs:label>delete</rdfs:label>
    <rdfs:domain rdf:resource="http://example.org/onto/class/google_compute_per_instance_config"/>
    <rdfs:range rdf:resource="http://www.w3.org/2001/XMLSchema#string"/>
  </owl:DatatypeProperty>
  <owl:DatatypeProperty rdf:about="http://example.org/onto/prop/google_compute_per_instance_config_update">
    <rdfs:label>update</rdfs:label>
    <rdfs:domain rdf:resource="http://example.org/onto/class/google_compute_per_instance_config"/>
    <rdfs:range rdf:resource="http://www.w3.org/2001/XMLSchema#string"/>
  </owl:DatatypeProperty>
</rdf:RDF>
