<?xml version="1.0" encoding="UTF-8"?>
<rdf:RDF
  xmlns:rdf="http://www.w3.org/1999/02/22-rdf-syntax-ns#"
  xmlns:rdfs="http://www.w3.org/2000/01/rdf-schema#"
  xmlns:owl="http://www.w3.org/2002/07/owl#"
  xmlns:xsd="http://www.w3.org/2001/XMLSchema#"
  xml:base="http://example.org/onto/">
  <owl:Class rdf:about="http://example.org/onto/class/google_developer_connect_account_connector">
    <rdfs:label>google_developer_connect_account_connector</rdfs:label>
    <rdfs:comment>#
#     ***     AUTO GENERATED CODE    ***    Type: MMv1     ***
#
# ----------------------------------------------------------------------------
#
#     This code is generated by Magic Modules using the following:
#
#     Configuration: https:#github.com/GoogleCloudPlatform/magic-modules/tree/main/mmv1/products/developerconnect/AccountConnector.yaml
#     Template:      https:#github.com/GoogleCloudPlatform/magic-modules/tree/main/mmv1/templates/terraform/resource.html.markdown.tmpl
#
#     DO NOT EDIT this file directly. Any changes made to this file will be
#     overwritten during the next generation cycle.
#
# ----------------------------------------------------------------------------
subcategory: "Developer Connect"
description: |-
  Description
---</rdfs:comment>
  </owl:Class>
  <owl:DatatypeProperty rdf:about="http://example.org/onto/prop/google_developer_connect_account_connector_account_connector_id">
    <rdfs:label>account_connector_id</rdfs:label>
    <rdfs:comment>Required. The ID to use for the AccountConnector, which will become the final
component of the AccountConnector's resource name. Its format should adhere
to https://google.aip.dev/122#resource-id-segments Names must be unique
per-project per-location.</rdfs:comment>
    <rdfs:domain rdf:resource="http://example.org/onto/class/google_developer_connect_account_connector"/>
    <rdfs:range rdf:resource="http://www.w3.org/2001/XMLSchema#string"/>
  </owl:DatatypeProperty>
  <owl:DatatypeProperty rdf:about="http://example.org/onto/prop/google_developer_connect_account_connector_annotations">
    <rdfs:label>annotations</rdfs:label>
    <rdfs:comment>Optional. Allows users to store small amounts of arbitrary data.

**Note**: This field is non-authoritative, and will only manage the annotations present in your configuration.
Please refer to the field 'effective_annotations' for all of the annotations present on the resource.</rdfs:comment>
    <rdfs:domain rdf:resource="http://example.org/onto/class/google_developer_connect_account_connector"/>
    <rdfs:range rdf:resource="http://www.w3.org/2001/XMLSchema#string"/>
  </owl:DatatypeProperty>
  <owl:DatatypeProperty rdf:about="http://example.org/onto/prop/google_developer_connect_account_connector_create_time">
    <rdfs:label>create_time</rdfs:label>
    <rdfs:comment>Output only. The timestamp when the userConnection was created.</rdfs:comment>
    <rdfs:domain rdf:resource="http://example.org/onto/class/google_developer_connect_account_connector"/>
    <rdfs:range rdf:resource="http://www.w3.org/2001/XMLSchema#string"/>
  </owl:DatatypeProperty>
  <owl:DatatypeProperty rdf:about="http://example.org/onto/prop/google_developer_connect_account_connector_effective_annotations">
    <rdfs:label>effective_annotations</rdfs:label>
    <rdfs:comment>All of annotations (key/value pairs) present on the resource in GCP, including the annotations configured through Terraform, other clients and services.</rdfs:comment>
    <rdfs:domain rdf:resource="http://example.org/onto/class/google_developer_connect_account_connector"/>
    <rdfs:range rdf:resource="http://www.w3.org/2001/XMLSchema#string"/>
  </owl:DatatypeProperty>
  <owl:DatatypeProperty rdf:about="http://example.org/onto/prop/google_developer_connect_account_connector_effective_labels">
    <rdfs:label>effective_labels</rdfs:label>
    <rdfs:comment>All of labels (key/value pairs) present on the resource in GCP, including the labels configured through Terraform, other clients and services.</rdfs:comment>
    <rdfs:domain rdf:resource="http://example.org/onto/class/google_developer_connect_account_connector"/>
    <rdfs:range rdf:resource="http://www.w3.org/2001/XMLSchema#string"/>
  </owl:DatatypeProperty>
  <owl:DatatypeProperty rdf:about="http://example.org/onto/prop/google_developer_connect_account_connector_id">
    <rdfs:label>id</rdfs:label>
    <rdfs:domain rdf:resource="http://example.org/onto/class/google_developer_connect_account_connector"/>
    <rdfs:range rdf:resource="http://www.w3.org/2001/XMLSchema#string"/>
  </owl:DatatypeProperty>
  <owl:DatatypeProperty rdf:about="http://example.org/onto/prop/google_developer_connect_account_connector_labels">
    <rdfs:label>labels</rdfs:label>
    <rdfs:comment>Optional. Labels as key value pairs

**Note**: This field is non-authoritative, and will only manage the labels present in your configuration.
Please refer to the field 'effective_labels' for all of the labels present on the resource.</rdfs:comment>
    <rdfs:domain rdf:resource="http://example.org/onto/class/google_developer_connect_account_connector"/>
    <rdfs:range rdf:resource="http://www.w3.org/2001/XMLSchema#string"/>
  </owl:DatatypeProperty>
  <owl:DatatypeProperty rdf:about="http://example.org/onto/prop/google_developer_connect_account_connector_location">
    <rdfs:label>location</rdfs:label>
    <rdfs:comment>The location of the resource.</rdfs:comment>
    <rdfs:domain rdf:resource="http://example.org/onto/class/google_developer_connect_account_connector"/>
    <rdfs:range rdf:resource="http://www.w3.org/2001/XMLSchema#string"/>
  </owl:DatatypeProperty>
  <owl:DatatypeProperty rdf:about="http://example.org/onto/prop/google_developer_connect_account_connector_name">
    <rdfs:label>name</rdfs:label>
    <rdfs:comment>Identifier. The resource name of the userConnection, in the format
'projects/{project}/locations/{location}/accountConnectors/{account_connector_id}'.</rdfs:comment>
    <rdfs:domain rdf:resource="http://example.org/onto/class/google_developer_connect_account_connector"/>
    <rdfs:range rdf:resource="http://www.w3.org/2001/XMLSchema#string"/>
  </owl:DatatypeProperty>
  <owl:DatatypeProperty rdf:about="http://example.org/onto/prop/google_developer_connect_account_connector_oauth_start_uri">
    <rdfs:label>oauth_start_uri</rdfs:label>
    <rdfs:comment>Output only. Start OAuth flow by clicking on this URL.</rdfs:comment>
    <rdfs:domain rdf:resource="http://example.org/onto/class/google_developer_connect_account_connector"/>
    <rdfs:range rdf:resource="http://www.w3.org/2001/XMLSchema#string"/>
  </owl:DatatypeProperty>
  <owl:DatatypeProperty rdf:about="http://example.org/onto/prop/google_developer_connect_account_connector_project">
    <rdfs:label>project</rdfs:label>
    <rdfs:domain rdf:resource="http://example.org/onto/class/google_developer_connect_account_connector"/>
    <rdfs:range rdf:resource="http://www.w3.org/2001/XMLSchema#string"/>
  </owl:DatatypeProperty>
  <owl:DatatypeProperty rdf:about="http://example.org/onto/prop/google_developer_connect_account_connector_terraform_labels">
    <rdfs:label>terraform_labels</rdfs:label>
    <rdfs:comment>The combination of labels configured directly on the resource
 and default labels configured on the provider.</rdfs:comment>
    <rdfs:domain rdf:resource="http://example.org/onto/class/google_developer_connect_account_connector"/>
    <rdfs:range rdf:resource="http://www.w3.org/2001/XMLSchema#string"/>
  </owl:DatatypeProperty>
  <owl:DatatypeProperty rdf:about="http://example.org/onto/prop/google_developer_connect_account_connector_update_time">
    <rdfs:label>update_time</rdfs:label>
    <rdfs:comment>Output only. The timestamp when the userConnection was updated.</rdfs:comment>
    <rdfs:domain rdf:resource="http://example.org/onto/class/google_developer_connect_account_connector"/>
    <rdfs:range rdf:resource="http://www.w3.org/2001/XMLSchema#string"/>
  </owl:DatatypeProperty>
  <owl:DatatypeProperty rdf:about="http://example.org/onto/prop/google_developer_connect_account_connector_scopes">
    <rdfs:label>scopes</rdfs:label>
    <rdfs:comment>Required. User selected scopes to apply to the Oauth config
In the event of changing scopes, user records under AccountConnector will
be deleted and users will re-auth again.</rdfs:comment>
    <rdfs:domain rdf:resource="http://example.org/onto/class/google_developer_connect_account_connector"/>
    <rdfs:range rdf:resource="http://www.w3.org/2001/XMLSchema#string"/>
  </owl:DatatypeProperty>
  <owl:DatatypeProperty rdf:about="http://example.org/onto/prop/google_developer_connect_account_connector_system_provider_id">
    <rdfs:label>system_provider_id</rdfs:label>
    <rdfs:comment>List of providers that are owned by Developer Connect.

Possible values:
GITHUB
GITLAB
GOOGLE
SENTRY
ROVO
NEW_RELIC
DATASTAX</rdfs:comment>
    <rdfs:domain rdf:resource="http://example.org/onto/class/google_developer_connect_account_connector"/>
    <rdfs:range rdf:resource="http://www.w3.org/2001/XMLSchema#string"/>
  </owl:DatatypeProperty>
  <owl:DatatypeProperty rdf:about="http://example.org/onto/prop/google_developer_connect_account_connector_create">
    <rdfs:label>create</rdfs:label>
    <rdfs:domain rdf:resource="http://example.org/onto/class/google_developer_connect_account_connector"/>
    <rdfs:range rdf:resource="http://www.w3.org/2001/XMLSchema#string"/>
  </owl:DatatypeProperty>
  <owl:DatatypeProperty rdf:about="http://example.org/onto/prop/google_developer_connect_account_connector_delete">
    <rdfs:label>delete</rdfs:label>
    <rdfs:domain rdf:resource="http://example.org/onto/class/google_developer_connect_account_connector"/>
    <rdfs:range rdf:resource="http://www.w3.org/2001/XMLSchema#string"/>
  </owl:DatatypeProperty>
  <owl:DatatypeProperty rdf:about="http://example.org/onto/prop/google_developer_connect_account_connector_update">
    <rdfs:label>update</rdfs:label>
    <rdfs:domain rdf:resource="http://example.org/onto/class/google_developer_connect_account_connector"/>
    <rdfs:range rdf:resource="http://www.w3.org/2001/XMLSchema#string"/>
  </owl:DatatypeProperty>
</rdf:RDF>
