<?xml version="1.0" encoding="UTF-8"?>
<rdf:RDF
  xmlns:rdf="http://www.w3.org/1999/02/22-rdf-syntax-ns#"
  xmlns:rdfs="http://www.w3.org/2000/01/rdf-schema#"
  xmlns:owl="http://www.w3.org/2002/07/owl#"
  xmlns:xsd="http://www.w3.org/2001/XMLSchema#"
  xml:base="http://example.org/onto/">
  <owl:Class rdf:about="http://example.org/onto/class/google_cloud_identity_group">
    <rdfs:label>google_cloud_identity_group</rdfs:label>
    <rdfs:comment>#
#     ***     AUTO GENERATED CODE    ***    Type: MMv1     ***
#
# ----------------------------------------------------------------------------
#
#     This code is generated by Magic Modules using the following:
#
#     Configuration: https:#github.com/GoogleCloudPlatform/magic-modules/tree/main/mmv1/products/cloudidentity/Group.yaml
#     Template:      https:#github.com/GoogleCloudPlatform/magic-modules/tree/main/mmv1/templates/terraform/resource.html.markdown.tmpl
#
#     DO NOT EDIT this file directly. Any changes made to this file will be
#     overwritten during the next generation cycle.
#
# ----------------------------------------------------------------------------
subcategory: "Cloud Identity"
description: |-
  A Cloud Identity resource representing a Group.
---</rdfs:comment>
  </owl:Class>
  <owl:DatatypeProperty rdf:about="http://example.org/onto/prop/google_cloud_identity_group_additional_group_keys">
    <rdfs:label>additional_group_keys</rdfs:label>
    <rdfs:comment>Additional group keys associated with the Group</rdfs:comment>
    <rdfs:domain rdf:resource="http://example.org/onto/class/google_cloud_identity_group"/>
    <rdfs:range rdf:resource="http://www.w3.org/2001/XMLSchema#string"/>
  </owl:DatatypeProperty>
  <owl:DatatypeProperty rdf:about="http://example.org/onto/prop/google_cloud_identity_group_create_time">
    <rdfs:label>create_time</rdfs:label>
    <rdfs:comment>The time when the Group was created.</rdfs:comment>
    <rdfs:domain rdf:resource="http://example.org/onto/class/google_cloud_identity_group"/>
    <rdfs:range rdf:resource="http://www.w3.org/2001/XMLSchema#string"/>
  </owl:DatatypeProperty>
  <owl:DatatypeProperty rdf:about="http://example.org/onto/prop/google_cloud_identity_group_description">
    <rdfs:label>description</rdfs:label>
    <rdfs:comment>An extended description to help users determine the purpose of a Group.
Must not be longer than 4,096 characters.</rdfs:comment>
    <rdfs:domain rdf:resource="http://example.org/onto/class/google_cloud_identity_group"/>
    <rdfs:range rdf:resource="http://www.w3.org/2001/XMLSchema#string"/>
  </owl:DatatypeProperty>
  <owl:DatatypeProperty rdf:about="http://example.org/onto/prop/google_cloud_identity_group_display_name">
    <rdfs:label>display_name</rdfs:label>
    <rdfs:comment>The display name of the Group.</rdfs:comment>
    <rdfs:domain rdf:resource="http://example.org/onto/class/google_cloud_identity_group"/>
    <rdfs:range rdf:resource="http://www.w3.org/2001/XMLSchema#string"/>
  </owl:DatatypeProperty>
  <owl:DatatypeProperty rdf:about="http://example.org/onto/prop/google_cloud_identity_group_id">
    <rdfs:label>id</rdfs:label>
    <rdfs:domain rdf:resource="http://example.org/onto/class/google_cloud_identity_group"/>
    <rdfs:range rdf:resource="http://www.w3.org/2001/XMLSchema#string"/>
  </owl:DatatypeProperty>
  <owl:DatatypeProperty rdf:about="http://example.org/onto/prop/google_cloud_identity_group_initial_group_config">
    <rdfs:label>initial_group_config</rdfs:label>
    <rdfs:comment>The initial configuration options for creating a Group.

See the
[API reference](https://cloud.google.com/identity/docs/reference/rest/v1beta1/groups/create#initialgroupconfig)
for possible values. Default value: "EMPTY" Possible values: ["INITIAL_GROUP_CONFIG_UNSPECIFIED", "WITH_INITIAL_OWNER", "EMPTY"]</rdfs:comment>
    <rdfs:domain rdf:resource="http://example.org/onto/class/google_cloud_identity_group"/>
    <rdfs:range rdf:resource="http://www.w3.org/2001/XMLSchema#string"/>
  </owl:DatatypeProperty>
  <owl:DatatypeProperty rdf:about="http://example.org/onto/prop/google_cloud_identity_group_labels">
    <rdfs:label>labels</rdfs:label>
    <rdfs:comment>One or more label entries that apply to the Group. Currently supported labels contain a key with an empty value.

Google Groups are the default type of group and have a label with a key of cloudidentity.googleapis.com/groups.discussion_forum and an empty value.

Existing Google Groups can have an additional label with a key of cloudidentity.googleapis.com/groups.security and an empty value added to them. This is an immutable change and the security label cannot be removed once added.

Dynamic groups have a label with a key of cloudidentity.googleapis.com/groups.dynamic.

Identity-mapped groups for Cloud Search have a label with a key of system/groups/external and an empty value.</rdfs:comment>
    <rdfs:domain rdf:resource="http://example.org/onto/class/google_cloud_identity_group"/>
    <rdfs:range rdf:resource="http://www.w3.org/2001/XMLSchema#string"/>
  </owl:DatatypeProperty>
  <owl:DatatypeProperty rdf:about="http://example.org/onto/prop/google_cloud_identity_group_name">
    <rdfs:label>name</rdfs:label>
    <rdfs:comment>Resource name of the Group in the format: groups/{group_id}, where group_id
is the unique ID assigned to the Group.</rdfs:comment>
    <rdfs:domain rdf:resource="http://example.org/onto/class/google_cloud_identity_group"/>
    <rdfs:range rdf:resource="http://www.w3.org/2001/XMLSchema#string"/>
  </owl:DatatypeProperty>
  <owl:DatatypeProperty rdf:about="http://example.org/onto/prop/google_cloud_identity_group_parent">
    <rdfs:label>parent</rdfs:label>
    <rdfs:comment>The resource name of the entity under which this Group resides in the
Cloud Identity resource hierarchy.

Must be of the form identitysources/{identity_source_id} for external-identity-mapped
groups or customers/{customer_id} for Google Groups.</rdfs:comment>
    <rdfs:domain rdf:resource="http://example.org/onto/class/google_cloud_identity_group"/>
    <rdfs:range rdf:resource="http://www.w3.org/2001/XMLSchema#string"/>
  </owl:DatatypeProperty>
  <owl:DatatypeProperty rdf:about="http://example.org/onto/prop/google_cloud_identity_group_update_time">
    <rdfs:label>update_time</rdfs:label>
    <rdfs:comment>The time when the Group was last updated.</rdfs:comment>
    <rdfs:domain rdf:resource="http://example.org/onto/class/google_cloud_identity_group"/>
    <rdfs:range rdf:resource="http://www.w3.org/2001/XMLSchema#string"/>
  </owl:DatatypeProperty>
  <owl:DatatypeProperty rdf:about="http://example.org/onto/prop/google_cloud_identity_group_id">
    <rdfs:label>id</rdfs:label>
    <rdfs:comment>The ID of the entity.

For Google-managed entities, the id must be the email address of an existing
group or user.

For external-identity-mapped entities, the id must be a string conforming
to the Identity Source's requirements.

Must be unique within a namespace.</rdfs:comment>
    <rdfs:domain rdf:resource="http://example.org/onto/class/google_cloud_identity_group"/>
    <rdfs:range rdf:resource="http://www.w3.org/2001/XMLSchema#string"/>
  </owl:DatatypeProperty>
  <owl:DatatypeProperty rdf:about="http://example.org/onto/prop/google_cloud_identity_group_namespace">
    <rdfs:label>namespace</rdfs:label>
    <rdfs:comment>The namespace in which the entity exists.

If not specified, the EntityKey represents a Google-managed entity
such as a Google user or a Google Group.

If specified, the EntityKey represents an external-identity-mapped group.
The namespace must correspond to an identity source created in Admin Console
and must be in the form of 'identitysources/{identity_source_id}'.</rdfs:comment>
    <rdfs:domain rdf:resource="http://example.org/onto/class/google_cloud_identity_group"/>
    <rdfs:range rdf:resource="http://www.w3.org/2001/XMLSchema#string"/>
  </owl:DatatypeProperty>
  <owl:DatatypeProperty rdf:about="http://example.org/onto/prop/google_cloud_identity_group_create">
    <rdfs:label>create</rdfs:label>
    <rdfs:domain rdf:resource="http://example.org/onto/class/google_cloud_identity_group"/>
    <rdfs:range rdf:resource="http://www.w3.org/2001/XMLSchema#string"/>
  </owl:DatatypeProperty>
  <owl:DatatypeProperty rdf:about="http://example.org/onto/prop/google_cloud_identity_group_delete">
    <rdfs:label>delete</rdfs:label>
    <rdfs:domain rdf:resource="http://example.org/onto/class/google_cloud_identity_group"/>
    <rdfs:range rdf:resource="http://www.w3.org/2001/XMLSchema#string"/>
  </owl:DatatypeProperty>
  <owl:DatatypeProperty rdf:about="http://example.org/onto/prop/google_cloud_identity_group_update">
    <rdfs:label>update</rdfs:label>
    <rdfs:domain rdf:resource="http://example.org/onto/class/google_cloud_identity_group"/>
    <rdfs:range rdf:resource="http://www.w3.org/2001/XMLSchema#string"/>
  </owl:DatatypeProperty>
</rdf:RDF>
