<?xml version="1.0" encoding="UTF-8"?>
<rdf:RDF
  xmlns:rdf="http://www.w3.org/1999/02/22-rdf-syntax-ns#"
  xmlns:rdfs="http://www.w3.org/2000/01/rdf-schema#"
  xmlns:owl="http://www.w3.org/2002/07/owl#"
  xmlns:xsd="http://www.w3.org/2001/XMLSchema#"
  xml:base="http://example.org/onto/">
  <owl:Class rdf:about="http://example.org/onto/class/google_cloudbuildv2_connection">
    <rdfs:label>google_cloudbuildv2_connection</rdfs:label>
    <rdfs:comment>#
#     ***     AUTO GENERATED CODE    ***    Type: MMv1     ***
#
# ----------------------------------------------------------------------------
#
#     This code is generated by Magic Modules using the following:
#
#     Configuration: https:#github.com/GoogleCloudPlatform/magic-modules/tree/main/mmv1/products/cloudbuildv2/Connection.yaml
#     Template:      https:#github.com/GoogleCloudPlatform/magic-modules/tree/main/mmv1/templates/terraform/resource.html.markdown.tmpl
#
#     DO NOT EDIT this file directly. Any changes made to this file will be
#     overwritten during the next generation cycle.
#
# ----------------------------------------------------------------------------
subcategory: "Cloud Build v2"
description: |-
  A connection to a SCM like GitHub, GitHub Enterprise, Bitbucket Data Center/Cloud or GitLab.
---</rdfs:comment>
  </owl:Class>
  <owl:DatatypeProperty rdf:about="http://example.org/onto/prop/google_cloudbuildv2_connection_annotations">
    <rdfs:label>annotations</rdfs:label>
    <rdfs:comment>Allows clients to store small amounts of arbitrary data.

**Note**: This field is non-authoritative, and will only manage the annotations present in your configuration.
Please refer to the field 'effective_annotations' for all of the annotations present on the resource.</rdfs:comment>
    <rdfs:domain rdf:resource="http://example.org/onto/class/google_cloudbuildv2_connection"/>
    <rdfs:range rdf:resource="http://www.w3.org/2001/XMLSchema#string"/>
  </owl:DatatypeProperty>
  <owl:DatatypeProperty rdf:about="http://example.org/onto/prop/google_cloudbuildv2_connection_create_time">
    <rdfs:label>create_time</rdfs:label>
    <rdfs:comment>Output only. Server assigned timestamp for when the connection was created.</rdfs:comment>
    <rdfs:domain rdf:resource="http://example.org/onto/class/google_cloudbuildv2_connection"/>
    <rdfs:range rdf:resource="http://www.w3.org/2001/XMLSchema#string"/>
  </owl:DatatypeProperty>
  <owl:DatatypeProperty rdf:about="http://example.org/onto/prop/google_cloudbuildv2_connection_disabled">
    <rdfs:label>disabled</rdfs:label>
    <rdfs:comment>If disabled is set to true, functionality is disabled for this connection. Repository based API methods and webhooks processing for repositories in this connection will be disabled.</rdfs:comment>
    <rdfs:domain rdf:resource="http://example.org/onto/class/google_cloudbuildv2_connection"/>
    <rdfs:range rdf:resource="http://www.w3.org/2001/XMLSchema#string"/>
  </owl:DatatypeProperty>
  <owl:DatatypeProperty rdf:about="http://example.org/onto/prop/google_cloudbuildv2_connection_effective_annotations">
    <rdfs:label>effective_annotations</rdfs:label>
    <rdfs:comment>All of annotations (key/value pairs) present on the resource in GCP, including the annotations configured through Terraform, other clients and services.</rdfs:comment>
    <rdfs:domain rdf:resource="http://example.org/onto/class/google_cloudbuildv2_connection"/>
    <rdfs:range rdf:resource="http://www.w3.org/2001/XMLSchema#string"/>
  </owl:DatatypeProperty>
  <owl:DatatypeProperty rdf:about="http://example.org/onto/prop/google_cloudbuildv2_connection_etag">
    <rdfs:label>etag</rdfs:label>
    <rdfs:comment>This checksum is computed by the server based on the value of other fields, and may be sent on update and delete requests to ensure the client has an up-to-date value before proceeding.</rdfs:comment>
    <rdfs:domain rdf:resource="http://example.org/onto/class/google_cloudbuildv2_connection"/>
    <rdfs:range rdf:resource="http://www.w3.org/2001/XMLSchema#string"/>
  </owl:DatatypeProperty>
  <owl:DatatypeProperty rdf:about="http://example.org/onto/prop/google_cloudbuildv2_connection_id">
    <rdfs:label>id</rdfs:label>
    <rdfs:domain rdf:resource="http://example.org/onto/class/google_cloudbuildv2_connection"/>
    <rdfs:range rdf:resource="http://www.w3.org/2001/XMLSchema#string"/>
  </owl:DatatypeProperty>
  <owl:DatatypeProperty rdf:about="http://example.org/onto/prop/google_cloudbuildv2_connection_installation_state">
    <rdfs:label>installation_state</rdfs:label>
    <rdfs:comment>Output only. Installation state of the Connection.</rdfs:comment>
    <rdfs:domain rdf:resource="http://example.org/onto/class/google_cloudbuildv2_connection"/>
    <rdfs:range rdf:resource="http://www.w3.org/2001/XMLSchema#string"/>
  </owl:DatatypeProperty>
  <owl:DatatypeProperty rdf:about="http://example.org/onto/prop/google_cloudbuildv2_connection_location">
    <rdfs:label>location</rdfs:label>
    <rdfs:comment>The location for the resource</rdfs:comment>
    <rdfs:domain rdf:resource="http://example.org/onto/class/google_cloudbuildv2_connection"/>
    <rdfs:range rdf:resource="http://www.w3.org/2001/XMLSchema#string"/>
  </owl:DatatypeProperty>
  <owl:DatatypeProperty rdf:about="http://example.org/onto/prop/google_cloudbuildv2_connection_name">
    <rdfs:label>name</rdfs:label>
    <rdfs:comment>Immutable. The resource name of the connection.</rdfs:comment>
    <rdfs:domain rdf:resource="http://example.org/onto/class/google_cloudbuildv2_connection"/>
    <rdfs:range rdf:resource="http://www.w3.org/2001/XMLSchema#string"/>
  </owl:DatatypeProperty>
  <owl:DatatypeProperty rdf:about="http://example.org/onto/prop/google_cloudbuildv2_connection_project">
    <rdfs:label>project</rdfs:label>
    <rdfs:domain rdf:resource="http://example.org/onto/class/google_cloudbuildv2_connection"/>
    <rdfs:range rdf:resource="http://www.w3.org/2001/XMLSchema#string"/>
  </owl:DatatypeProperty>
  <owl:DatatypeProperty rdf:about="http://example.org/onto/prop/google_cloudbuildv2_connection_reconciling">
    <rdfs:label>reconciling</rdfs:label>
    <rdfs:comment>Output only. Set to true when the connection is being set up or updated in the background.</rdfs:comment>
    <rdfs:domain rdf:resource="http://example.org/onto/class/google_cloudbuildv2_connection"/>
    <rdfs:range rdf:resource="http://www.w3.org/2001/XMLSchema#string"/>
  </owl:DatatypeProperty>
  <owl:DatatypeProperty rdf:about="http://example.org/onto/prop/google_cloudbuildv2_connection_update_time">
    <rdfs:label>update_time</rdfs:label>
    <rdfs:comment>Output only. Server assigned timestamp for when the connection was updated.</rdfs:comment>
    <rdfs:domain rdf:resource="http://example.org/onto/class/google_cloudbuildv2_connection"/>
    <rdfs:range rdf:resource="http://www.w3.org/2001/XMLSchema#string"/>
  </owl:DatatypeProperty>
  <owl:DatatypeProperty rdf:about="http://example.org/onto/prop/google_cloudbuildv2_connection_webhook_secret_secret_version">
    <rdfs:label>webhook_secret_secret_version</rdfs:label>
    <rdfs:comment>Required. Immutable. SecretManager resource containing the webhook secret used to verify webhook events, formatted as 'projects/*/secrets/*/versions/*'.</rdfs:comment>
    <rdfs:domain rdf:resource="http://example.org/onto/class/google_cloudbuildv2_connection"/>
    <rdfs:range rdf:resource="http://www.w3.org/2001/XMLSchema#string"/>
  </owl:DatatypeProperty>
  <owl:DatatypeProperty rdf:about="http://example.org/onto/prop/google_cloudbuildv2_connection_workspace">
    <rdfs:label>workspace</rdfs:label>
    <rdfs:comment>The Bitbucket Cloud Workspace ID to be connected to Google Cloud Platform.</rdfs:comment>
    <rdfs:domain rdf:resource="http://example.org/onto/class/google_cloudbuildv2_connection"/>
    <rdfs:range rdf:resource="http://www.w3.org/2001/XMLSchema#string"/>
  </owl:DatatypeProperty>
  <owl:DatatypeProperty rdf:about="http://example.org/onto/prop/google_cloudbuildv2_connection_user_token_secret_version">
    <rdfs:label>user_token_secret_version</rdfs:label>
    <rdfs:comment>Required. A SecretManager resource containing the user token that authorizes the Cloud Build connection. Format: 'projects/*/secrets/*/versions/*'.</rdfs:comment>
    <rdfs:domain rdf:resource="http://example.org/onto/class/google_cloudbuildv2_connection"/>
    <rdfs:range rdf:resource="http://www.w3.org/2001/XMLSchema#string"/>
  </owl:DatatypeProperty>
  <owl:DatatypeProperty rdf:about="http://example.org/onto/prop/google_cloudbuildv2_connection_username">
    <rdfs:label>username</rdfs:label>
    <rdfs:comment>Output only. The username associated to this token.</rdfs:comment>
    <rdfs:domain rdf:resource="http://example.org/onto/class/google_cloudbuildv2_connection"/>
    <rdfs:range rdf:resource="http://www.w3.org/2001/XMLSchema#string"/>
  </owl:DatatypeProperty>
  <owl:DatatypeProperty rdf:about="http://example.org/onto/prop/google_cloudbuildv2_connection_user_token_secret_version">
    <rdfs:label>user_token_secret_version</rdfs:label>
    <rdfs:comment>Required. A SecretManager resource containing the user token that authorizes the Cloud Build connection. Format: 'projects/*/secrets/*/versions/*'.</rdfs:comment>
    <rdfs:domain rdf:resource="http://example.org/onto/class/google_cloudbuildv2_connection"/>
    <rdfs:range rdf:resource="http://www.w3.org/2001/XMLSchema#string"/>
  </owl:DatatypeProperty>
  <owl:DatatypeProperty rdf:about="http://example.org/onto/prop/google_cloudbuildv2_connection_username">
    <rdfs:label>username</rdfs:label>
    <rdfs:comment>Output only. The username associated to this token.</rdfs:comment>
    <rdfs:domain rdf:resource="http://example.org/onto/class/google_cloudbuildv2_connection"/>
    <rdfs:range rdf:resource="http://www.w3.org/2001/XMLSchema#string"/>
  </owl:DatatypeProperty>
  <owl:DatatypeProperty rdf:about="http://example.org/onto/prop/google_cloudbuildv2_connection_host_uri">
    <rdfs:label>host_uri</rdfs:label>
    <rdfs:comment>The URI of the Bitbucket Data Center host this connection is for.</rdfs:comment>
    <rdfs:domain rdf:resource="http://example.org/onto/class/google_cloudbuildv2_connection"/>
    <rdfs:range rdf:resource="http://www.w3.org/2001/XMLSchema#string"/>
  </owl:DatatypeProperty>
  <owl:DatatypeProperty rdf:about="http://example.org/onto/prop/google_cloudbuildv2_connection_server_version">
    <rdfs:label>server_version</rdfs:label>
    <rdfs:comment>Output only. Version of the Bitbucket Data Center running on the 'host_uri'.</rdfs:comment>
    <rdfs:domain rdf:resource="http://example.org/onto/class/google_cloudbuildv2_connection"/>
    <rdfs:range rdf:resource="http://www.w3.org/2001/XMLSchema#string"/>
  </owl:DatatypeProperty>
  <owl:DatatypeProperty rdf:about="http://example.org/onto/prop/google_cloudbuildv2_connection_ssl_ca">
    <rdfs:label>ssl_ca</rdfs:label>
    <rdfs:comment>SSL certificate to use for requests to the Bitbucket Data Center.</rdfs:comment>
    <rdfs:domain rdf:resource="http://example.org/onto/class/google_cloudbuildv2_connection"/>
    <rdfs:range rdf:resource="http://www.w3.org/2001/XMLSchema#string"/>
  </owl:DatatypeProperty>
  <owl:DatatypeProperty rdf:about="http://example.org/onto/prop/google_cloudbuildv2_connection_webhook_secret_secret_version">
    <rdfs:label>webhook_secret_secret_version</rdfs:label>
    <rdfs:comment>Required. Immutable. SecretManager resource containing the webhook secret used to verify webhook events, formatted as 'projects/*/secrets/*/versions/*'.</rdfs:comment>
    <rdfs:domain rdf:resource="http://example.org/onto/class/google_cloudbuildv2_connection"/>
    <rdfs:range rdf:resource="http://www.w3.org/2001/XMLSchema#string"/>
  </owl:DatatypeProperty>
  <owl:DatatypeProperty rdf:about="http://example.org/onto/prop/google_cloudbuildv2_connection_user_token_secret_version">
    <rdfs:label>user_token_secret_version</rdfs:label>
    <rdfs:comment>Required. A SecretManager resource containing the user token that authorizes the Cloud Build connection. Format: 'projects/*/secrets/*/versions/*'.</rdfs:comment>
    <rdfs:domain rdf:resource="http://example.org/onto/class/google_cloudbuildv2_connection"/>
    <rdfs:range rdf:resource="http://www.w3.org/2001/XMLSchema#string"/>
  </owl:DatatypeProperty>
  <owl:DatatypeProperty rdf:about="http://example.org/onto/prop/google_cloudbuildv2_connection_username">
    <rdfs:label>username</rdfs:label>
    <rdfs:comment>Output only. The username associated to this token.</rdfs:comment>
    <rdfs:domain rdf:resource="http://example.org/onto/class/google_cloudbuildv2_connection"/>
    <rdfs:range rdf:resource="http://www.w3.org/2001/XMLSchema#string"/>
  </owl:DatatypeProperty>
  <owl:DatatypeProperty rdf:about="http://example.org/onto/prop/google_cloudbuildv2_connection_user_token_secret_version">
    <rdfs:label>user_token_secret_version</rdfs:label>
    <rdfs:comment>Required. A SecretManager resource containing the user token that authorizes the Cloud Build connection. Format: 'projects/*/secrets/*/versions/*'.</rdfs:comment>
    <rdfs:domain rdf:resource="http://example.org/onto/class/google_cloudbuildv2_connection"/>
    <rdfs:range rdf:resource="http://www.w3.org/2001/XMLSchema#string"/>
  </owl:DatatypeProperty>
  <owl:DatatypeProperty rdf:about="http://example.org/onto/prop/google_cloudbuildv2_connection_username">
    <rdfs:label>username</rdfs:label>
    <rdfs:comment>Output only. The username associated to this token.</rdfs:comment>
    <rdfs:domain rdf:resource="http://example.org/onto/class/google_cloudbuildv2_connection"/>
    <rdfs:range rdf:resource="http://www.w3.org/2001/XMLSchema#string"/>
  </owl:DatatypeProperty>
  <owl:DatatypeProperty rdf:about="http://example.org/onto/prop/google_cloudbuildv2_connection_service">
    <rdfs:label>service</rdfs:label>
    <rdfs:comment>Required. The Service Directory service name. Format: projects/{project}/locations/{location}/namespaces/{namespace}/services/{service}.</rdfs:comment>
    <rdfs:domain rdf:resource="http://example.org/onto/class/google_cloudbuildv2_connection"/>
    <rdfs:range rdf:resource="http://www.w3.org/2001/XMLSchema#string"/>
  </owl:DatatypeProperty>
  <owl:DatatypeProperty rdf:about="http://example.org/onto/prop/google_cloudbuildv2_connection_app_installation_id">
    <rdfs:label>app_installation_id</rdfs:label>
    <rdfs:comment>GitHub App installation id.</rdfs:comment>
    <rdfs:domain rdf:resource="http://example.org/onto/class/google_cloudbuildv2_connection"/>
    <rdfs:range rdf:resource="http://www.w3.org/2001/XMLSchema#string"/>
  </owl:DatatypeProperty>
  <owl:DatatypeProperty rdf:about="http://example.org/onto/prop/google_cloudbuildv2_connection_oauth_token_secret_version">
    <rdfs:label>oauth_token_secret_version</rdfs:label>
    <rdfs:comment>A SecretManager resource containing the OAuth token that authorizes the Cloud Build connection. Format: 'projects/*/secrets/*/versions/*'.</rdfs:comment>
    <rdfs:domain rdf:resource="http://example.org/onto/class/google_cloudbuildv2_connection"/>
    <rdfs:range rdf:resource="http://www.w3.org/2001/XMLSchema#string"/>
  </owl:DatatypeProperty>
  <owl:DatatypeProperty rdf:about="http://example.org/onto/prop/google_cloudbuildv2_connection_username">
    <rdfs:label>username</rdfs:label>
    <rdfs:comment>Output only. The username associated to this token.</rdfs:comment>
    <rdfs:domain rdf:resource="http://example.org/onto/class/google_cloudbuildv2_connection"/>
    <rdfs:range rdf:resource="http://www.w3.org/2001/XMLSchema#string"/>
  </owl:DatatypeProperty>
  <owl:DatatypeProperty rdf:about="http://example.org/onto/prop/google_cloudbuildv2_connection_app_id">
    <rdfs:label>app_id</rdfs:label>
    <rdfs:comment>Id of the GitHub App created from the manifest.</rdfs:comment>
    <rdfs:domain rdf:resource="http://example.org/onto/class/google_cloudbuildv2_connection"/>
    <rdfs:range rdf:resource="http://www.w3.org/2001/XMLSchema#string"/>
  </owl:DatatypeProperty>
  <owl:DatatypeProperty rdf:about="http://example.org/onto/prop/google_cloudbuildv2_connection_app_installation_id">
    <rdfs:label>app_installation_id</rdfs:label>
    <rdfs:comment>ID of the installation of the GitHub App.</rdfs:comment>
    <rdfs:domain rdf:resource="http://example.org/onto/class/google_cloudbuildv2_connection"/>
    <rdfs:range rdf:resource="http://www.w3.org/2001/XMLSchema#string"/>
  </owl:DatatypeProperty>
  <owl:DatatypeProperty rdf:about="http://example.org/onto/prop/google_cloudbuildv2_connection_app_slug">
    <rdfs:label>app_slug</rdfs:label>
    <rdfs:comment>The URL-friendly name of the GitHub App.</rdfs:comment>
    <rdfs:domain rdf:resource="http://example.org/onto/class/google_cloudbuildv2_connection"/>
    <rdfs:range rdf:resource="http://www.w3.org/2001/XMLSchema#string"/>
  </owl:DatatypeProperty>
  <owl:DatatypeProperty rdf:about="http://example.org/onto/prop/google_cloudbuildv2_connection_host_uri">
    <rdfs:label>host_uri</rdfs:label>
    <rdfs:comment>Required. The URI of the GitHub Enterprise host this connection is for.</rdfs:comment>
    <rdfs:domain rdf:resource="http://example.org/onto/class/google_cloudbuildv2_connection"/>
    <rdfs:range rdf:resource="http://www.w3.org/2001/XMLSchema#string"/>
  </owl:DatatypeProperty>
  <owl:DatatypeProperty rdf:about="http://example.org/onto/prop/google_cloudbuildv2_connection_private_key_secret_version">
    <rdfs:label>private_key_secret_version</rdfs:label>
    <rdfs:comment>SecretManager resource containing the private key of the GitHub App, formatted as 'projects/*/secrets/*/versions/*'.</rdfs:comment>
    <rdfs:domain rdf:resource="http://example.org/onto/class/google_cloudbuildv2_connection"/>
    <rdfs:range rdf:resource="http://www.w3.org/2001/XMLSchema#string"/>
  </owl:DatatypeProperty>
  <owl:DatatypeProperty rdf:about="http://example.org/onto/prop/google_cloudbuildv2_connection_ssl_ca">
    <rdfs:label>ssl_ca</rdfs:label>
    <rdfs:comment>SSL certificate to use for requests to GitHub Enterprise.</rdfs:comment>
    <rdfs:domain rdf:resource="http://example.org/onto/class/google_cloudbuildv2_connection"/>
    <rdfs:range rdf:resource="http://www.w3.org/2001/XMLSchema#string"/>
  </owl:DatatypeProperty>
  <owl:DatatypeProperty rdf:about="http://example.org/onto/prop/google_cloudbuildv2_connection_webhook_secret_secret_version">
    <rdfs:label>webhook_secret_secret_version</rdfs:label>
    <rdfs:comment>SecretManager resource containing the webhook secret of the GitHub App, formatted as 'projects/*/secrets/*/versions/*'.</rdfs:comment>
    <rdfs:domain rdf:resource="http://example.org/onto/class/google_cloudbuildv2_connection"/>
    <rdfs:range rdf:resource="http://www.w3.org/2001/XMLSchema#string"/>
  </owl:DatatypeProperty>
  <owl:DatatypeProperty rdf:about="http://example.org/onto/prop/google_cloudbuildv2_connection_service">
    <rdfs:label>service</rdfs:label>
    <rdfs:comment>Required. The Service Directory service name. Format: projects/{project}/locations/{location}/namespaces/{namespace}/services/{service}.</rdfs:comment>
    <rdfs:domain rdf:resource="http://example.org/onto/class/google_cloudbuildv2_connection"/>
    <rdfs:range rdf:resource="http://www.w3.org/2001/XMLSchema#string"/>
  </owl:DatatypeProperty>
  <owl:DatatypeProperty rdf:about="http://example.org/onto/prop/google_cloudbuildv2_connection_host_uri">
    <rdfs:label>host_uri</rdfs:label>
    <rdfs:comment>The URI of the GitLab Enterprise host this connection is for. If not specified, the default value is https://gitlab.com.</rdfs:comment>
    <rdfs:domain rdf:resource="http://example.org/onto/class/google_cloudbuildv2_connection"/>
    <rdfs:range rdf:resource="http://www.w3.org/2001/XMLSchema#string"/>
  </owl:DatatypeProperty>
  <owl:DatatypeProperty rdf:about="http://example.org/onto/prop/google_cloudbuildv2_connection_server_version">
    <rdfs:label>server_version</rdfs:label>
    <rdfs:comment>Output only. Version of the GitLab Enterprise server running on the 'host_uri'.</rdfs:comment>
    <rdfs:domain rdf:resource="http://example.org/onto/class/google_cloudbuildv2_connection"/>
    <rdfs:range rdf:resource="http://www.w3.org/2001/XMLSchema#string"/>
  </owl:DatatypeProperty>
  <owl:DatatypeProperty rdf:about="http://example.org/onto/prop/google_cloudbuildv2_connection_ssl_ca">
    <rdfs:label>ssl_ca</rdfs:label>
    <rdfs:comment>SSL certificate to use for requests to GitLab Enterprise.</rdfs:comment>
    <rdfs:domain rdf:resource="http://example.org/onto/class/google_cloudbuildv2_connection"/>
    <rdfs:range rdf:resource="http://www.w3.org/2001/XMLSchema#string"/>
  </owl:DatatypeProperty>
  <owl:DatatypeProperty rdf:about="http://example.org/onto/prop/google_cloudbuildv2_connection_webhook_secret_secret_version">
    <rdfs:label>webhook_secret_secret_version</rdfs:label>
    <rdfs:comment>Required. Immutable. SecretManager resource containing the webhook secret of a GitLab Enterprise project, formatted as 'projects/*/secrets/*/versions/*'.</rdfs:comment>
    <rdfs:domain rdf:resource="http://example.org/onto/class/google_cloudbuildv2_connection"/>
    <rdfs:range rdf:resource="http://www.w3.org/2001/XMLSchema#string"/>
  </owl:DatatypeProperty>
  <owl:DatatypeProperty rdf:about="http://example.org/onto/prop/google_cloudbuildv2_connection_user_token_secret_version">
    <rdfs:label>user_token_secret_version</rdfs:label>
    <rdfs:comment>Required. A SecretManager resource containing the user token that authorizes the Cloud Build connection. Format: 'projects/*/secrets/*/versions/*'.</rdfs:comment>
    <rdfs:domain rdf:resource="http://example.org/onto/class/google_cloudbuildv2_connection"/>
    <rdfs:range rdf:resource="http://www.w3.org/2001/XMLSchema#string"/>
  </owl:DatatypeProperty>
  <owl:DatatypeProperty rdf:about="http://example.org/onto/prop/google_cloudbuildv2_connection_username">
    <rdfs:label>username</rdfs:label>
    <rdfs:comment>Output only. The username associated to this token.</rdfs:comment>
    <rdfs:domain rdf:resource="http://example.org/onto/class/google_cloudbuildv2_connection"/>
    <rdfs:range rdf:resource="http://www.w3.org/2001/XMLSchema#string"/>
  </owl:DatatypeProperty>
  <owl:DatatypeProperty rdf:about="http://example.org/onto/prop/google_cloudbuildv2_connection_user_token_secret_version">
    <rdfs:label>user_token_secret_version</rdfs:label>
    <rdfs:comment>Required. A SecretManager resource containing the user token that authorizes the Cloud Build connection. Format: 'projects/*/secrets/*/versions/*'.</rdfs:comment>
    <rdfs:domain rdf:resource="http://example.org/onto/class/google_cloudbuildv2_connection"/>
    <rdfs:range rdf:resource="http://www.w3.org/2001/XMLSchema#string"/>
  </owl:DatatypeProperty>
  <owl:DatatypeProperty rdf:about="http://example.org/onto/prop/google_cloudbuildv2_connection_username">
    <rdfs:label>username</rdfs:label>
    <rdfs:comment>Output only. The username associated to this token.</rdfs:comment>
    <rdfs:domain rdf:resource="http://example.org/onto/class/google_cloudbuildv2_connection"/>
    <rdfs:range rdf:resource="http://www.w3.org/2001/XMLSchema#string"/>
  </owl:DatatypeProperty>
  <owl:DatatypeProperty rdf:about="http://example.org/onto/prop/google_cloudbuildv2_connection_service">
    <rdfs:label>service</rdfs:label>
    <rdfs:comment>Required. The Service Directory service name. Format: projects/{project}/locations/{location}/namespaces/{namespace}/services/{service}.</rdfs:comment>
    <rdfs:domain rdf:resource="http://example.org/onto/class/google_cloudbuildv2_connection"/>
    <rdfs:range rdf:resource="http://www.w3.org/2001/XMLSchema#string"/>
  </owl:DatatypeProperty>
  <owl:DatatypeProperty rdf:about="http://example.org/onto/prop/google_cloudbuildv2_connection_create">
    <rdfs:label>create</rdfs:label>
    <rdfs:domain rdf:resource="http://example.org/onto/class/google_cloudbuildv2_connection"/>
    <rdfs:range rdf:resource="http://www.w3.org/2001/XMLSchema#string"/>
  </owl:DatatypeProperty>
  <owl:DatatypeProperty rdf:about="http://example.org/onto/prop/google_cloudbuildv2_connection_delete">
    <rdfs:label>delete</rdfs:label>
    <rdfs:domain rdf:resource="http://example.org/onto/class/google_cloudbuildv2_connection"/>
    <rdfs:range rdf:resource="http://www.w3.org/2001/XMLSchema#string"/>
  </owl:DatatypeProperty>
  <owl:DatatypeProperty rdf:about="http://example.org/onto/prop/google_cloudbuildv2_connection_update">
    <rdfs:label>update</rdfs:label>
    <rdfs:domain rdf:resource="http://example.org/onto/class/google_cloudbuildv2_connection"/>
    <rdfs:range rdf:resource="http://www.w3.org/2001/XMLSchema#string"/>
  </owl:DatatypeProperty>
</rdf:RDF>
