<?xml version="1.0" encoding="UTF-8"?>
<rdf:RDF
  xmlns:rdf="http://www.w3.org/1999/02/22-rdf-syntax-ns#"
  xmlns:rdfs="http://www.w3.org/2000/01/rdf-schema#"
  xmlns:owl="http://www.w3.org/2002/07/owl#"
  xmlns:xsd="http://www.w3.org/2001/XMLSchema#"
  xml:base="http://example.org/onto/">
  <owl:Class rdf:about="http://example.org/onto/class/google_healthcare_dicom_store">
    <rdfs:label>google_healthcare_dicom_store</rdfs:label>
    <rdfs:comment>#
#     ***     AUTO GENERATED CODE    ***    Type: MMv1     ***
#
# ----------------------------------------------------------------------------
#
#     This code is generated by Magic Modules using the following:
#
#     Configuration: https:#github.com/GoogleCloudPlatform/magic-modules/tree/main/mmv1/products/healthcare/DicomStore.yaml
#     Template:      https:#github.com/GoogleCloudPlatform/magic-modules/tree/main/mmv1/templates/terraform/resource.html.markdown.tmpl
#
#     DO NOT EDIT this file directly. Any changes made to this file will be
#     overwritten during the next generation cycle.
#
# ----------------------------------------------------------------------------
subcategory: "Cloud Healthcare"
description: |-
  A DicomStore is a datastore inside a Healthcare dataset that conforms to the DICOM
  (https://www.
---</rdfs:comment>
  </owl:Class>
  <owl:DatatypeProperty rdf:about="http://example.org/onto/prop/google_healthcare_dicom_store_dataset">
    <rdfs:label>dataset</rdfs:label>
    <rdfs:comment>Identifies the dataset addressed by this request. Must be in the format
'projects/{project}/locations/{location}/datasets/{dataset}'</rdfs:comment>
    <rdfs:domain rdf:resource="http://example.org/onto/class/google_healthcare_dicom_store"/>
    <rdfs:range rdf:resource="http://www.w3.org/2001/XMLSchema#string"/>
  </owl:DatatypeProperty>
  <owl:DatatypeProperty rdf:about="http://example.org/onto/prop/google_healthcare_dicom_store_effective_labels">
    <rdfs:label>effective_labels</rdfs:label>
    <rdfs:comment>All of labels (key/value pairs) present on the resource in GCP, including the labels configured through Terraform, other clients and services.</rdfs:comment>
    <rdfs:domain rdf:resource="http://example.org/onto/class/google_healthcare_dicom_store"/>
    <rdfs:range rdf:resource="http://www.w3.org/2001/XMLSchema#string"/>
  </owl:DatatypeProperty>
  <owl:DatatypeProperty rdf:about="http://example.org/onto/prop/google_healthcare_dicom_store_id">
    <rdfs:label>id</rdfs:label>
    <rdfs:domain rdf:resource="http://example.org/onto/class/google_healthcare_dicom_store"/>
    <rdfs:range rdf:resource="http://www.w3.org/2001/XMLSchema#string"/>
  </owl:DatatypeProperty>
  <owl:DatatypeProperty rdf:about="http://example.org/onto/prop/google_healthcare_dicom_store_labels">
    <rdfs:label>labels</rdfs:label>
    <rdfs:comment>User-supplied key-value pairs used to organize DICOM stores.

Label keys must be between 1 and 63 characters long, have a UTF-8 encoding of maximum 128 bytes, and must
conform to the following PCRE regular expression: [\p{Ll}\p{Lo}][\p{Ll}\p{Lo}\p{N}_-]{0,62}

Label values are optional, must be between 1 and 63 characters long, have a UTF-8 encoding of maximum 128
bytes, and must conform to the following PCRE regular expression: [\p{Ll}\p{Lo}\p{N}_-]{0,63}

No more than 64 labels can be associated with a given store.

An object containing a list of "key": value pairs.
Example: { "name": "wrench", "mass": "1.3kg", "count": "3" }.


**Note**: This field is non-authoritative, and will only manage the labels present in your configuration.
Please refer to the field 'effective_labels' for all of the labels present on the resource.</rdfs:comment>
    <rdfs:domain rdf:resource="http://example.org/onto/class/google_healthcare_dicom_store"/>
    <rdfs:range rdf:resource="http://www.w3.org/2001/XMLSchema#string"/>
  </owl:DatatypeProperty>
  <owl:DatatypeProperty rdf:about="http://example.org/onto/prop/google_healthcare_dicom_store_name">
    <rdfs:label>name</rdfs:label>
    <rdfs:comment>The resource name for the DicomStore.

** Changing this property may recreate the Dicom store (removing all data) **</rdfs:comment>
    <rdfs:domain rdf:resource="http://example.org/onto/class/google_healthcare_dicom_store"/>
    <rdfs:range rdf:resource="http://www.w3.org/2001/XMLSchema#string"/>
  </owl:DatatypeProperty>
  <owl:DatatypeProperty rdf:about="http://example.org/onto/prop/google_healthcare_dicom_store_self_link">
    <rdfs:label>self_link</rdfs:label>
    <rdfs:comment>The fully qualified name of this dataset</rdfs:comment>
    <rdfs:domain rdf:resource="http://example.org/onto/class/google_healthcare_dicom_store"/>
    <rdfs:range rdf:resource="http://www.w3.org/2001/XMLSchema#string"/>
  </owl:DatatypeProperty>
  <owl:DatatypeProperty rdf:about="http://example.org/onto/prop/google_healthcare_dicom_store_terraform_labels">
    <rdfs:label>terraform_labels</rdfs:label>
    <rdfs:comment>The combination of labels configured directly on the resource
 and default labels configured on the provider.</rdfs:comment>
    <rdfs:domain rdf:resource="http://example.org/onto/class/google_healthcare_dicom_store"/>
    <rdfs:range rdf:resource="http://www.w3.org/2001/XMLSchema#string"/>
  </owl:DatatypeProperty>
  <owl:DatatypeProperty rdf:about="http://example.org/onto/prop/google_healthcare_dicom_store_pubsub_topic">
    <rdfs:label>pubsub_topic</rdfs:label>
    <rdfs:comment>The Cloud Pub/Sub topic that notifications of changes are published on. Supplied by the client.
PubsubMessage.Data will contain the resource name. PubsubMessage.MessageId is the ID of this message.
It is guaranteed to be unique within the topic. PubsubMessage.PublishTime is the time at which the message
was published. Notifications are only sent if the topic is non-empty. Topic names must be scoped to a
project. service-PROJECT_NUMBER@gcp-sa-healthcare.iam.gserviceaccount.com must have publisher permissions on the given
Cloud Pub/Sub topic. Not having adequate permissions will cause the calls that send notifications to fail.</rdfs:comment>
    <rdfs:domain rdf:resource="http://example.org/onto/class/google_healthcare_dicom_store"/>
    <rdfs:range rdf:resource="http://www.w3.org/2001/XMLSchema#string"/>
  </owl:DatatypeProperty>
  <owl:DatatypeProperty rdf:about="http://example.org/onto/prop/google_healthcare_dicom_store_send_for_bulk_import">
    <rdfs:label>send_for_bulk_import</rdfs:label>
    <rdfs:comment>Indicates whether or not to send Pub/Sub notifications on bulk import. Only supported for DICOM imports.</rdfs:comment>
    <rdfs:domain rdf:resource="http://example.org/onto/class/google_healthcare_dicom_store"/>
    <rdfs:range rdf:resource="http://www.w3.org/2001/XMLSchema#string"/>
  </owl:DatatypeProperty>
  <owl:DatatypeProperty rdf:about="http://example.org/onto/prop/google_healthcare_dicom_store_create">
    <rdfs:label>create</rdfs:label>
    <rdfs:domain rdf:resource="http://example.org/onto/class/google_healthcare_dicom_store"/>
    <rdfs:range rdf:resource="http://www.w3.org/2001/XMLSchema#string"/>
  </owl:DatatypeProperty>
  <owl:DatatypeProperty rdf:about="http://example.org/onto/prop/google_healthcare_dicom_store_delete">
    <rdfs:label>delete</rdfs:label>
    <rdfs:domain rdf:resource="http://example.org/onto/class/google_healthcare_dicom_store"/>
    <rdfs:range rdf:resource="http://www.w3.org/2001/XMLSchema#string"/>
  </owl:DatatypeProperty>
  <owl:DatatypeProperty rdf:about="http://example.org/onto/prop/google_healthcare_dicom_store_update">
    <rdfs:label>update</rdfs:label>
    <rdfs:domain rdf:resource="http://example.org/onto/class/google_healthcare_dicom_store"/>
    <rdfs:range rdf:resource="http://www.w3.org/2001/XMLSchema#string"/>
  </owl:DatatypeProperty>
</rdf:RDF>
