<?xml version="1.0" encoding="UTF-8"?>
<rdf:RDF
  xmlns:rdf="http://www.w3.org/1999/02/22-rdf-syntax-ns#"
  xmlns:rdfs="http://www.w3.org/2000/01/rdf-schema#"
  xmlns:owl="http://www.w3.org/2002/07/owl#"
  xmlns:xsd="http://www.w3.org/2001/XMLSchema#"
  xml:base="http://example.org/onto/">
  <owl:Class rdf:about="http://example.org/onto/class/google_access_context_manager_service_perimeters">
    <rdfs:label>google_access_context_manager_service_perimeters</rdfs:label>
    <rdfs:comment>#
#     ***     AUTO GENERATED CODE    ***    Type: MMv1     ***
#
# ----------------------------------------------------------------------------
#
#     This code is generated by Magic Modules using the following:
#
#     Configuration: https:#github.com/GoogleCloudPlatform/magic-modules/tree/main/mmv1/products/accesscontextmanager/ServicePerimeters.yaml
#     Template:      https:#github.com/GoogleCloudPlatform/magic-modules/tree/main/mmv1/templates/terraform/resource.html.markdown.tmpl
#
#     DO NOT EDIT this file directly. Any changes made to this file will be
#     overwritten during the next generation cycle.
#
# ----------------------------------------------------------------------------
subcategory: "Access Context Manager (VPC Service Controls)"
description: |-
  Replace all existing Service Perimeters in an Access Policy with the Service Perimeters provided.
---</rdfs:comment>
  </owl:Class>
  <owl:DatatypeProperty rdf:about="http://example.org/onto/prop/google_access_context_manager_service_perimeters_id">
    <rdfs:label>id</rdfs:label>
    <rdfs:domain rdf:resource="http://example.org/onto/class/google_access_context_manager_service_perimeters"/>
    <rdfs:range rdf:resource="http://www.w3.org/2001/XMLSchema#string"/>
  </owl:DatatypeProperty>
  <owl:DatatypeProperty rdf:about="http://example.org/onto/prop/google_access_context_manager_service_perimeters_parent">
    <rdfs:label>parent</rdfs:label>
    <rdfs:comment>The AccessPolicy this ServicePerimeter lives in.
Format: accessPolicies/{policy_id}</rdfs:comment>
    <rdfs:domain rdf:resource="http://example.org/onto/class/google_access_context_manager_service_perimeters"/>
    <rdfs:range rdf:resource="http://www.w3.org/2001/XMLSchema#string"/>
  </owl:DatatypeProperty>
  <owl:DatatypeProperty rdf:about="http://example.org/onto/prop/google_access_context_manager_service_perimeters_create_time">
    <rdfs:label>create_time</rdfs:label>
    <rdfs:comment>Time the AccessPolicy was created in UTC.</rdfs:comment>
    <rdfs:domain rdf:resource="http://example.org/onto/class/google_access_context_manager_service_perimeters"/>
    <rdfs:range rdf:resource="http://www.w3.org/2001/XMLSchema#string"/>
  </owl:DatatypeProperty>
  <owl:DatatypeProperty rdf:about="http://example.org/onto/prop/google_access_context_manager_service_perimeters_description">
    <rdfs:label>description</rdfs:label>
    <rdfs:comment>Description of the ServicePerimeter and its use. Does not affect
behavior.</rdfs:comment>
    <rdfs:domain rdf:resource="http://example.org/onto/class/google_access_context_manager_service_perimeters"/>
    <rdfs:range rdf:resource="http://www.w3.org/2001/XMLSchema#string"/>
  </owl:DatatypeProperty>
  <owl:DatatypeProperty rdf:about="http://example.org/onto/prop/google_access_context_manager_service_perimeters_name">
    <rdfs:label>name</rdfs:label>
    <rdfs:comment>Resource name for the ServicePerimeter. The short_name component must
begin with a letter and only include alphanumeric and '_'.
Format: accessPolicies/{policy_id}/servicePerimeters/{short_name}</rdfs:comment>
    <rdfs:domain rdf:resource="http://example.org/onto/class/google_access_context_manager_service_perimeters"/>
    <rdfs:range rdf:resource="http://www.w3.org/2001/XMLSchema#string"/>
  </owl:DatatypeProperty>
  <owl:DatatypeProperty rdf:about="http://example.org/onto/prop/google_access_context_manager_service_perimeters_perimeter_type">
    <rdfs:label>perimeter_type</rdfs:label>
    <rdfs:comment>Specifies the type of the Perimeter. There are two types: regular and
bridge. Regular Service Perimeter contains resources, access levels,
and restricted services. Every resource can be in at most
ONE regular Service Perimeter.

In addition to being in a regular service perimeter, a resource can also
be in zero or more perimeter bridges. A perimeter bridge only contains
resources. Cross project operations are permitted if all effected
resources share some perimeter (whether bridge or regular). Perimeter
Bridge does not contain access levels or services: those are governed
entirely by the regular perimeter that resource is in.

Perimeter Bridges are typically useful when building more complex
topologies with many independent perimeters that need to share some data
with a common perimeter, but should not be able to share data among
themselves. Default value: "PERIMETER_TYPE_REGULAR" Possible values: ["PERIMETER_TYPE_REGULAR", "PERIMETER_TYPE_BRIDGE"]</rdfs:comment>
    <rdfs:domain rdf:resource="http://example.org/onto/class/google_access_context_manager_service_perimeters"/>
    <rdfs:range rdf:resource="http://www.w3.org/2001/XMLSchema#string"/>
  </owl:DatatypeProperty>
  <owl:DatatypeProperty rdf:about="http://example.org/onto/prop/google_access_context_manager_service_perimeters_title">
    <rdfs:label>title</rdfs:label>
    <rdfs:comment>Human readable title. Must be unique within the Policy.</rdfs:comment>
    <rdfs:domain rdf:resource="http://example.org/onto/class/google_access_context_manager_service_perimeters"/>
    <rdfs:range rdf:resource="http://www.w3.org/2001/XMLSchema#string"/>
  </owl:DatatypeProperty>
  <owl:DatatypeProperty rdf:about="http://example.org/onto/prop/google_access_context_manager_service_perimeters_update_time">
    <rdfs:label>update_time</rdfs:label>
    <rdfs:comment>Time the AccessPolicy was updated in UTC.</rdfs:comment>
    <rdfs:domain rdf:resource="http://example.org/onto/class/google_access_context_manager_service_perimeters"/>
    <rdfs:range rdf:resource="http://www.w3.org/2001/XMLSchema#string"/>
  </owl:DatatypeProperty>
  <owl:DatatypeProperty rdf:about="http://example.org/onto/prop/google_access_context_manager_service_perimeters_use_explicit_dry_run_spec">
    <rdfs:label>use_explicit_dry_run_spec</rdfs:label>
    <rdfs:comment>Use explicit dry run spec flag. Ordinarily, a dry-run spec implicitly exists
for all Service Perimeters, and that spec is identical to the status for those
Service Perimeters. When this flag is set, it inhibits the generation of the
implicit spec, thereby allowing the user to explicitly provide a
configuration ("spec") to use in a dry-run version of the Service Perimeter.
This allows the user to test changes to the enforced config ("status") without
actually enforcing them. This testing is done through analyzing the differences
between currently enforced and suggested restrictions. useExplicitDryRunSpec must
bet set to True if any of the fields in the spec are set to non-default values.</rdfs:comment>
    <rdfs:domain rdf:resource="http://example.org/onto/class/google_access_context_manager_service_perimeters"/>
    <rdfs:range rdf:resource="http://www.w3.org/2001/XMLSchema#string"/>
  </owl:DatatypeProperty>
  <owl:DatatypeProperty rdf:about="http://example.org/onto/prop/google_access_context_manager_service_perimeters_access_levels">
    <rdfs:label>access_levels</rdfs:label>
    <rdfs:comment>A list of AccessLevel resource names that allow resources within
the ServicePerimeter to be accessed from the internet.
AccessLevels listed must be in the same policy as this
ServicePerimeter. Referencing a nonexistent AccessLevel is a
syntax error. If no AccessLevel names are listed, resources within
the perimeter can only be accessed via GCP calls with request
origins within the perimeter. For Service Perimeter Bridge, must
be empty.

Format: accessPolicies/{policy_id}/accessLevels/{access_level_name}</rdfs:comment>
    <rdfs:domain rdf:resource="http://example.org/onto/class/google_access_context_manager_service_perimeters"/>
    <rdfs:range rdf:resource="http://www.w3.org/2001/XMLSchema#string"/>
  </owl:DatatypeProperty>
  <owl:DatatypeProperty rdf:about="http://example.org/onto/prop/google_access_context_manager_service_perimeters_resources">
    <rdfs:label>resources</rdfs:label>
    <rdfs:comment>A list of GCP resources that are inside of the service perimeter.
Currently only projects are allowed.
Format: projects/{project_number}</rdfs:comment>
    <rdfs:domain rdf:resource="http://example.org/onto/class/google_access_context_manager_service_perimeters"/>
    <rdfs:range rdf:resource="http://www.w3.org/2001/XMLSchema#string"/>
  </owl:DatatypeProperty>
  <owl:DatatypeProperty rdf:about="http://example.org/onto/prop/google_access_context_manager_service_perimeters_restricted_services">
    <rdfs:label>restricted_services</rdfs:label>
    <rdfs:comment>GCP services that are subject to the Service Perimeter
restrictions. Must contain a list of services. For example, if
'storage.googleapis.com' is specified, access to the storage
buckets inside the perimeter must meet the perimeter's access
restrictions.</rdfs:comment>
    <rdfs:domain rdf:resource="http://example.org/onto/class/google_access_context_manager_service_perimeters"/>
    <rdfs:range rdf:resource="http://www.w3.org/2001/XMLSchema#string"/>
  </owl:DatatypeProperty>
  <owl:DatatypeProperty rdf:about="http://example.org/onto/prop/google_access_context_manager_service_perimeters_title">
    <rdfs:label>title</rdfs:label>
    <rdfs:comment>Human readable title. Must be unique within the perimeter. Does not affect behavior.</rdfs:comment>
    <rdfs:domain rdf:resource="http://example.org/onto/class/google_access_context_manager_service_perimeters"/>
    <rdfs:range rdf:resource="http://www.w3.org/2001/XMLSchema#string"/>
  </owl:DatatypeProperty>
  <owl:DatatypeProperty rdf:about="http://example.org/onto/prop/google_access_context_manager_service_perimeters_identities">
    <rdfs:label>identities</rdfs:label>
    <rdfs:comment>Identities can be an individual user, service account, Google group,
or third-party identity. For third-party identity, only single identities
are supported and other identity types are not supported.The v1 identities
that have the prefix user, group and serviceAccount in
https://cloud.google.com/iam/docs/principal-identifiers#v1 are supported.</rdfs:comment>
    <rdfs:domain rdf:resource="http://example.org/onto/class/google_access_context_manager_service_perimeters"/>
    <rdfs:range rdf:resource="http://www.w3.org/2001/XMLSchema#string"/>
  </owl:DatatypeProperty>
  <owl:DatatypeProperty rdf:about="http://example.org/onto/prop/google_access_context_manager_service_perimeters_identity_type">
    <rdfs:label>identity_type</rdfs:label>
    <rdfs:comment>Specifies the type of identities that are allowed access to outside the
perimeter. If left unspecified, then members of 'identities' field will
be allowed access. Possible values: ["IDENTITY_TYPE_UNSPECIFIED", "ANY_IDENTITY", "ANY_USER_ACCOUNT", "ANY_SERVICE_ACCOUNT"]</rdfs:comment>
    <rdfs:domain rdf:resource="http://example.org/onto/class/google_access_context_manager_service_perimeters"/>
    <rdfs:range rdf:resource="http://www.w3.org/2001/XMLSchema#string"/>
  </owl:DatatypeProperty>
  <owl:DatatypeProperty rdf:about="http://example.org/onto/prop/google_access_context_manager_service_perimeters_source_restriction">
    <rdfs:label>source_restriction</rdfs:label>
    <rdfs:comment>Whether to enforce traffic restrictions based on 'sources' field. If the 'sources' field is non-empty, then this field must be set to 'SOURCE_RESTRICTION_ENABLED'. Possible values: ["SOURCE_RESTRICTION_UNSPECIFIED", "SOURCE_RESTRICTION_ENABLED", "SOURCE_RESTRICTION_DISABLED"]</rdfs:comment>
    <rdfs:domain rdf:resource="http://example.org/onto/class/google_access_context_manager_service_perimeters"/>
    <rdfs:range rdf:resource="http://www.w3.org/2001/XMLSchema#string"/>
  </owl:DatatypeProperty>
  <owl:DatatypeProperty rdf:about="http://example.org/onto/prop/google_access_context_manager_service_perimeters_access_level">
    <rdfs:label>access_level</rdfs:label>
    <rdfs:comment>An AccessLevel resource name that allows resources outside the ServicePerimeter to be accessed from the inside.</rdfs:comment>
    <rdfs:domain rdf:resource="http://example.org/onto/class/google_access_context_manager_service_perimeters"/>
    <rdfs:range rdf:resource="http://www.w3.org/2001/XMLSchema#string"/>
  </owl:DatatypeProperty>
  <owl:DatatypeProperty rdf:about="http://example.org/onto/prop/google_access_context_manager_service_perimeters_resource">
    <rdfs:label>resource</rdfs:label>
    <rdfs:comment>A Google Cloud resource that is allowed to egress the perimeter.
Requests from these resources are allowed to access data outside the perimeter.
Currently only projects are allowed. Project format: 'projects/{project_number}'.
The resource may be in any Google Cloud organization, not just the
organization that the perimeter is defined in. '*' is not allowed, the
case of allowing all Google Cloud resources only is not supported.</rdfs:comment>
    <rdfs:domain rdf:resource="http://example.org/onto/class/google_access_context_manager_service_perimeters"/>
    <rdfs:range rdf:resource="http://www.w3.org/2001/XMLSchema#string"/>
  </owl:DatatypeProperty>
  <owl:DatatypeProperty rdf:about="http://example.org/onto/prop/google_access_context_manager_service_perimeters_external_resources">
    <rdfs:label>external_resources</rdfs:label>
    <rdfs:comment>A list of external resources that are allowed to be accessed. A request
matches if it contains an external resource in this list (Example:
s3://bucket/path). Currently '*' is not allowed.</rdfs:comment>
    <rdfs:domain rdf:resource="http://example.org/onto/class/google_access_context_manager_service_perimeters"/>
    <rdfs:range rdf:resource="http://www.w3.org/2001/XMLSchema#string"/>
  </owl:DatatypeProperty>
  <owl:DatatypeProperty rdf:about="http://example.org/onto/prop/google_access_context_manager_service_perimeters_resources">
    <rdfs:label>resources</rdfs:label>
    <rdfs:comment>A list of resources, currently only projects in the form
'projects/<projectnumber>', that match this to stanza. A request matches
if it contains a resource in this list. If * is specified for resources,
then this 'EgressTo' rule will authorize access to all resources outside
the perimeter.</rdfs:comment>
    <rdfs:domain rdf:resource="http://example.org/onto/class/google_access_context_manager_service_perimeters"/>
    <rdfs:range rdf:resource="http://www.w3.org/2001/XMLSchema#string"/>
  </owl:DatatypeProperty>
  <owl:DatatypeProperty rdf:about="http://example.org/onto/prop/google_access_context_manager_service_perimeters_roles">
    <rdfs:label>roles</rdfs:label>
    <rdfs:comment>A list of IAM roles that represent the set of operations that the sources
specified in the corresponding 'EgressFrom'
are allowed to perform.</rdfs:comment>
    <rdfs:domain rdf:resource="http://example.org/onto/class/google_access_context_manager_service_perimeters"/>
    <rdfs:range rdf:resource="http://www.w3.org/2001/XMLSchema#string"/>
  </owl:DatatypeProperty>
  <owl:DatatypeProperty rdf:about="http://example.org/onto/prop/google_access_context_manager_service_perimeters_service_name">
    <rdfs:label>service_name</rdfs:label>
    <rdfs:comment>The name of the API whose methods or permissions the 'IngressPolicy' or
'EgressPolicy' want to allow. A single 'ApiOperation' with serviceName
field set to '*' will allow all methods AND permissions for all services.</rdfs:comment>
    <rdfs:domain rdf:resource="http://example.org/onto/class/google_access_context_manager_service_perimeters"/>
    <rdfs:range rdf:resource="http://www.w3.org/2001/XMLSchema#string"/>
  </owl:DatatypeProperty>
  <owl:DatatypeProperty rdf:about="http://example.org/onto/prop/google_access_context_manager_service_perimeters_method">
    <rdfs:label>method</rdfs:label>
    <rdfs:comment>Value for 'method' should be a valid method name for the corresponding
'serviceName' in 'ApiOperation'. If '*' used as value for method,
then ALL methods and permissions are allowed.</rdfs:comment>
    <rdfs:domain rdf:resource="http://example.org/onto/class/google_access_context_manager_service_perimeters"/>
    <rdfs:range rdf:resource="http://www.w3.org/2001/XMLSchema#string"/>
  </owl:DatatypeProperty>
  <owl:DatatypeProperty rdf:about="http://example.org/onto/prop/google_access_context_manager_service_perimeters_permission">
    <rdfs:label>permission</rdfs:label>
    <rdfs:comment>Value for permission should be a valid Cloud IAM permission for the
corresponding 'serviceName' in 'ApiOperation'.</rdfs:comment>
    <rdfs:domain rdf:resource="http://example.org/onto/class/google_access_context_manager_service_perimeters"/>
    <rdfs:range rdf:resource="http://www.w3.org/2001/XMLSchema#string"/>
  </owl:DatatypeProperty>
  <owl:DatatypeProperty rdf:about="http://example.org/onto/prop/google_access_context_manager_service_perimeters_title">
    <rdfs:label>title</rdfs:label>
    <rdfs:comment>Human readable title. Must be unique within the perimeter. Does not affect behavior.</rdfs:comment>
    <rdfs:domain rdf:resource="http://example.org/onto/class/google_access_context_manager_service_perimeters"/>
    <rdfs:range rdf:resource="http://www.w3.org/2001/XMLSchema#string"/>
  </owl:DatatypeProperty>
  <owl:DatatypeProperty rdf:about="http://example.org/onto/prop/google_access_context_manager_service_perimeters_identities">
    <rdfs:label>identities</rdfs:label>
    <rdfs:comment>A list of identities that are allowed access through this ingress policy.
Should be in the format of email address. The email address should represent
individual user or service account only.</rdfs:comment>
    <rdfs:domain rdf:resource="http://example.org/onto/class/google_access_context_manager_service_perimeters"/>
    <rdfs:range rdf:resource="http://www.w3.org/2001/XMLSchema#string"/>
  </owl:DatatypeProperty>
  <owl:DatatypeProperty rdf:about="http://example.org/onto/prop/google_access_context_manager_service_perimeters_identity_type">
    <rdfs:label>identity_type</rdfs:label>
    <rdfs:comment>Specifies the type of identities that are allowed access from outside the
perimeter. If left unspecified, then members of 'identities' field will be
allowed access. Possible values: ["IDENTITY_TYPE_UNSPECIFIED", "ANY_IDENTITY", "ANY_USER_ACCOUNT", "ANY_SERVICE_ACCOUNT"]</rdfs:comment>
    <rdfs:domain rdf:resource="http://example.org/onto/class/google_access_context_manager_service_perimeters"/>
    <rdfs:range rdf:resource="http://www.w3.org/2001/XMLSchema#string"/>
  </owl:DatatypeProperty>
  <owl:DatatypeProperty rdf:about="http://example.org/onto/prop/google_access_context_manager_service_perimeters_access_level">
    <rdfs:label>access_level</rdfs:label>
    <rdfs:comment>An 'AccessLevel' resource name that allow resources within the
'ServicePerimeters' to be accessed from the internet. 'AccessLevels' listed
must be in the same policy as this 'ServicePerimeter'. Referencing a nonexistent
'AccessLevel' will cause an error. If no 'AccessLevel' names are listed,
resources within the perimeter can only be accessed via Google Cloud calls
with request origins within the perimeter.
Example 'accessPolicies/MY_POLICY/accessLevels/MY_LEVEL.'
If * is specified, then all IngressSources will be allowed.</rdfs:comment>
    <rdfs:domain rdf:resource="http://example.org/onto/class/google_access_context_manager_service_perimeters"/>
    <rdfs:range rdf:resource="http://www.w3.org/2001/XMLSchema#string"/>
  </owl:DatatypeProperty>
  <owl:DatatypeProperty rdf:about="http://example.org/onto/prop/google_access_context_manager_service_perimeters_resource">
    <rdfs:label>resource</rdfs:label>
    <rdfs:comment>A Google Cloud resource that is allowed to ingress the perimeter.
Requests from these resources will be allowed to access perimeter data.
Currently only projects are allowed. Format 'projects/{project_number}'
The project may be in any Google Cloud organization, not just the
organization that the perimeter is defined in. '*' is not allowed, the case
of allowing all Google Cloud resources only is not supported.</rdfs:comment>
    <rdfs:domain rdf:resource="http://example.org/onto/class/google_access_context_manager_service_perimeters"/>
    <rdfs:range rdf:resource="http://www.w3.org/2001/XMLSchema#string"/>
  </owl:DatatypeProperty>
  <owl:DatatypeProperty rdf:about="http://example.org/onto/prop/google_access_context_manager_service_perimeters_resources">
    <rdfs:label>resources</rdfs:label>
    <rdfs:comment>A list of resources, currently only projects in the form
'projects/<projectnumber>', protected by this 'ServicePerimeter'
that are allowed to be accessed by sources defined in the
corresponding 'IngressFrom'. A request matches if it contains
a resource in this list. If '*' is specified for resources,
then this 'IngressTo' rule will authorize access to all
resources inside the perimeter, provided that the request
also matches the 'operations' field.</rdfs:comment>
    <rdfs:domain rdf:resource="http://example.org/onto/class/google_access_context_manager_service_perimeters"/>
    <rdfs:range rdf:resource="http://www.w3.org/2001/XMLSchema#string"/>
  </owl:DatatypeProperty>
  <owl:DatatypeProperty rdf:about="http://example.org/onto/prop/google_access_context_manager_service_perimeters_roles">
    <rdfs:label>roles</rdfs:label>
    <rdfs:comment>A list of IAM roles that represent the set of operations that the sources
specified in the corresponding 'IngressFrom'
are allowed to perform.</rdfs:comment>
    <rdfs:domain rdf:resource="http://example.org/onto/class/google_access_context_manager_service_perimeters"/>
    <rdfs:range rdf:resource="http://www.w3.org/2001/XMLSchema#string"/>
  </owl:DatatypeProperty>
  <owl:DatatypeProperty rdf:about="http://example.org/onto/prop/google_access_context_manager_service_perimeters_service_name">
    <rdfs:label>service_name</rdfs:label>
    <rdfs:comment>The name of the API whose methods or permissions the 'IngressPolicy' or
'EgressPolicy' want to allow. A single 'ApiOperation' with 'serviceName'
field set to '*' will allow all methods AND permissions for all services.</rdfs:comment>
    <rdfs:domain rdf:resource="http://example.org/onto/class/google_access_context_manager_service_perimeters"/>
    <rdfs:range rdf:resource="http://www.w3.org/2001/XMLSchema#string"/>
  </owl:DatatypeProperty>
  <owl:DatatypeProperty rdf:about="http://example.org/onto/prop/google_access_context_manager_service_perimeters_method">
    <rdfs:label>method</rdfs:label>
    <rdfs:comment>Value for method should be a valid method name for the corresponding
serviceName in 'ApiOperation'. If '*' used as value for 'method', then
ALL methods and permissions are allowed.</rdfs:comment>
    <rdfs:domain rdf:resource="http://example.org/onto/class/google_access_context_manager_service_perimeters"/>
    <rdfs:range rdf:resource="http://www.w3.org/2001/XMLSchema#string"/>
  </owl:DatatypeProperty>
  <owl:DatatypeProperty rdf:about="http://example.org/onto/prop/google_access_context_manager_service_perimeters_permission">
    <rdfs:label>permission</rdfs:label>
    <rdfs:comment>Value for permission should be a valid Cloud IAM permission for the
corresponding 'serviceName' in 'ApiOperation'.</rdfs:comment>
    <rdfs:domain rdf:resource="http://example.org/onto/class/google_access_context_manager_service_perimeters"/>
    <rdfs:range rdf:resource="http://www.w3.org/2001/XMLSchema#string"/>
  </owl:DatatypeProperty>
  <owl:DatatypeProperty rdf:about="http://example.org/onto/prop/google_access_context_manager_service_perimeters_allowed_services">
    <rdfs:label>allowed_services</rdfs:label>
    <rdfs:comment>The list of APIs usable within the Service Perimeter.
Must be empty unless 'enableRestriction' is True.</rdfs:comment>
    <rdfs:domain rdf:resource="http://example.org/onto/class/google_access_context_manager_service_perimeters"/>
    <rdfs:range rdf:resource="http://www.w3.org/2001/XMLSchema#string"/>
  </owl:DatatypeProperty>
  <owl:DatatypeProperty rdf:about="http://example.org/onto/prop/google_access_context_manager_service_perimeters_enable_restriction">
    <rdfs:label>enable_restriction</rdfs:label>
    <rdfs:comment>Whether to restrict API calls within the Service Perimeter to the
list of APIs specified in 'allowedServices'.</rdfs:comment>
    <rdfs:domain rdf:resource="http://example.org/onto/class/google_access_context_manager_service_perimeters"/>
    <rdfs:range rdf:resource="http://www.w3.org/2001/XMLSchema#string"/>
  </owl:DatatypeProperty>
  <owl:DatatypeProperty rdf:about="http://example.org/onto/prop/google_access_context_manager_service_perimeters_access_levels">
    <rdfs:label>access_levels</rdfs:label>
    <rdfs:comment>A list of AccessLevel resource names that allow resources within
the ServicePerimeter to be accessed from the internet.
AccessLevels listed must be in the same policy as this
ServicePerimeter. Referencing a nonexistent AccessLevel is a
syntax error. If no AccessLevel names are listed, resources within
the perimeter can only be accessed via GCP calls with request
origins within the perimeter. For Service Perimeter Bridge, must
be empty.

Format: accessPolicies/{policy_id}/accessLevels/{access_level_name}</rdfs:comment>
    <rdfs:domain rdf:resource="http://example.org/onto/class/google_access_context_manager_service_perimeters"/>
    <rdfs:range rdf:resource="http://www.w3.org/2001/XMLSchema#string"/>
  </owl:DatatypeProperty>
  <owl:DatatypeProperty rdf:about="http://example.org/onto/prop/google_access_context_manager_service_perimeters_resources">
    <rdfs:label>resources</rdfs:label>
    <rdfs:comment>A list of GCP resources that are inside of the service perimeter.
Currently only projects are allowed.
Format: projects/{project_number}</rdfs:comment>
    <rdfs:domain rdf:resource="http://example.org/onto/class/google_access_context_manager_service_perimeters"/>
    <rdfs:range rdf:resource="http://www.w3.org/2001/XMLSchema#string"/>
  </owl:DatatypeProperty>
  <owl:DatatypeProperty rdf:about="http://example.org/onto/prop/google_access_context_manager_service_perimeters_restricted_services">
    <rdfs:label>restricted_services</rdfs:label>
    <rdfs:comment>GCP services that are subject to the Service Perimeter
restrictions. Must contain a list of services. For example, if
'storage.googleapis.com' is specified, access to the storage
buckets inside the perimeter must meet the perimeter's access
restrictions.</rdfs:comment>
    <rdfs:domain rdf:resource="http://example.org/onto/class/google_access_context_manager_service_perimeters"/>
    <rdfs:range rdf:resource="http://www.w3.org/2001/XMLSchema#string"/>
  </owl:DatatypeProperty>
  <owl:DatatypeProperty rdf:about="http://example.org/onto/prop/google_access_context_manager_service_perimeters_title">
    <rdfs:label>title</rdfs:label>
    <rdfs:comment>Human readable title. Must be unique within the perimeter. Does not affect behavior.</rdfs:comment>
    <rdfs:domain rdf:resource="http://example.org/onto/class/google_access_context_manager_service_perimeters"/>
    <rdfs:range rdf:resource="http://www.w3.org/2001/XMLSchema#string"/>
  </owl:DatatypeProperty>
  <owl:DatatypeProperty rdf:about="http://example.org/onto/prop/google_access_context_manager_service_perimeters_identities">
    <rdfs:label>identities</rdfs:label>
    <rdfs:comment>A list of identities that are allowed access through this 'EgressPolicy'.
Should be in the format of email address. The email address should
represent individual user or service account only.</rdfs:comment>
    <rdfs:domain rdf:resource="http://example.org/onto/class/google_access_context_manager_service_perimeters"/>
    <rdfs:range rdf:resource="http://www.w3.org/2001/XMLSchema#string"/>
  </owl:DatatypeProperty>
  <owl:DatatypeProperty rdf:about="http://example.org/onto/prop/google_access_context_manager_service_perimeters_identity_type">
    <rdfs:label>identity_type</rdfs:label>
    <rdfs:comment>Specifies the type of identities that are allowed access to outside the
perimeter. If left unspecified, then members of 'identities' field will
be allowed access. Possible values: ["IDENTITY_TYPE_UNSPECIFIED", "ANY_IDENTITY", "ANY_USER_ACCOUNT", "ANY_SERVICE_ACCOUNT"]</rdfs:comment>
    <rdfs:domain rdf:resource="http://example.org/onto/class/google_access_context_manager_service_perimeters"/>
    <rdfs:range rdf:resource="http://www.w3.org/2001/XMLSchema#string"/>
  </owl:DatatypeProperty>
  <owl:DatatypeProperty rdf:about="http://example.org/onto/prop/google_access_context_manager_service_perimeters_source_restriction">
    <rdfs:label>source_restriction</rdfs:label>
    <rdfs:comment>Whether to enforce traffic restrictions based on 'sources' field. If the 'sources' field is non-empty, then this field must be set to 'SOURCE_RESTRICTION_ENABLED'. Possible values: ["SOURCE_RESTRICTION_UNSPECIFIED", "SOURCE_RESTRICTION_ENABLED", "SOURCE_RESTRICTION_DISABLED"]</rdfs:comment>
    <rdfs:domain rdf:resource="http://example.org/onto/class/google_access_context_manager_service_perimeters"/>
    <rdfs:range rdf:resource="http://www.w3.org/2001/XMLSchema#string"/>
  </owl:DatatypeProperty>
  <owl:DatatypeProperty rdf:about="http://example.org/onto/prop/google_access_context_manager_service_perimeters_access_level">
    <rdfs:label>access_level</rdfs:label>
    <rdfs:comment>An AccessLevel resource name that allows resources outside the ServicePerimeter to be accessed from the inside.</rdfs:comment>
    <rdfs:domain rdf:resource="http://example.org/onto/class/google_access_context_manager_service_perimeters"/>
    <rdfs:range rdf:resource="http://www.w3.org/2001/XMLSchema#string"/>
  </owl:DatatypeProperty>
  <owl:DatatypeProperty rdf:about="http://example.org/onto/prop/google_access_context_manager_service_perimeters_resource">
    <rdfs:label>resource</rdfs:label>
    <rdfs:comment>A Google Cloud resource that is allowed to egress the perimeter.
Requests from these resources are allowed to access data outside the perimeter.
Currently only projects are allowed. Project format: 'projects/{project_number}'.
The resource may be in any Google Cloud organization, not just the
organization that the perimeter is defined in. '*' is not allowed, the
case of allowing all Google Cloud resources only is not supported.</rdfs:comment>
    <rdfs:domain rdf:resource="http://example.org/onto/class/google_access_context_manager_service_perimeters"/>
    <rdfs:range rdf:resource="http://www.w3.org/2001/XMLSchema#string"/>
  </owl:DatatypeProperty>
  <owl:DatatypeProperty rdf:about="http://example.org/onto/prop/google_access_context_manager_service_perimeters_external_resources">
    <rdfs:label>external_resources</rdfs:label>
    <rdfs:comment>A list of external resources that are allowed to be accessed. A request
matches if it contains an external resource in this list (Example:
s3://bucket/path). Currently '*' is not allowed.</rdfs:comment>
    <rdfs:domain rdf:resource="http://example.org/onto/class/google_access_context_manager_service_perimeters"/>
    <rdfs:range rdf:resource="http://www.w3.org/2001/XMLSchema#string"/>
  </owl:DatatypeProperty>
  <owl:DatatypeProperty rdf:about="http://example.org/onto/prop/google_access_context_manager_service_perimeters_resources">
    <rdfs:label>resources</rdfs:label>
    <rdfs:comment>A list of resources, currently only projects in the form
'projects/<projectnumber>', that match this to stanza. A request matches
if it contains a resource in this list. If * is specified for resources,
then this 'EgressTo' rule will authorize access to all resources outside
the perimeter.</rdfs:comment>
    <rdfs:domain rdf:resource="http://example.org/onto/class/google_access_context_manager_service_perimeters"/>
    <rdfs:range rdf:resource="http://www.w3.org/2001/XMLSchema#string"/>
  </owl:DatatypeProperty>
  <owl:DatatypeProperty rdf:about="http://example.org/onto/prop/google_access_context_manager_service_perimeters_roles">
    <rdfs:label>roles</rdfs:label>
    <rdfs:comment>A list of IAM roles that represent the set of operations that the sources
specified in the corresponding 'EgressFrom'
are allowed to perform.</rdfs:comment>
    <rdfs:domain rdf:resource="http://example.org/onto/class/google_access_context_manager_service_perimeters"/>
    <rdfs:range rdf:resource="http://www.w3.org/2001/XMLSchema#string"/>
  </owl:DatatypeProperty>
  <owl:DatatypeProperty rdf:about="http://example.org/onto/prop/google_access_context_manager_service_perimeters_service_name">
    <rdfs:label>service_name</rdfs:label>
    <rdfs:comment>The name of the API whose methods or permissions the 'IngressPolicy' or
'EgressPolicy' want to allow. A single 'ApiOperation' with serviceName
field set to '*' will allow all methods AND permissions for all services.</rdfs:comment>
    <rdfs:domain rdf:resource="http://example.org/onto/class/google_access_context_manager_service_perimeters"/>
    <rdfs:range rdf:resource="http://www.w3.org/2001/XMLSchema#string"/>
  </owl:DatatypeProperty>
  <owl:DatatypeProperty rdf:about="http://example.org/onto/prop/google_access_context_manager_service_perimeters_method">
    <rdfs:label>method</rdfs:label>
    <rdfs:comment>Value for 'method' should be a valid method name for the corresponding
'serviceName' in 'ApiOperation'. If '*' used as value for method,
then ALL methods and permissions are allowed.</rdfs:comment>
    <rdfs:domain rdf:resource="http://example.org/onto/class/google_access_context_manager_service_perimeters"/>
    <rdfs:range rdf:resource="http://www.w3.org/2001/XMLSchema#string"/>
  </owl:DatatypeProperty>
  <owl:DatatypeProperty rdf:about="http://example.org/onto/prop/google_access_context_manager_service_perimeters_permission">
    <rdfs:label>permission</rdfs:label>
    <rdfs:comment>Value for permission should be a valid Cloud IAM permission for the
corresponding 'serviceName' in 'ApiOperation'.</rdfs:comment>
    <rdfs:domain rdf:resource="http://example.org/onto/class/google_access_context_manager_service_perimeters"/>
    <rdfs:range rdf:resource="http://www.w3.org/2001/XMLSchema#string"/>
  </owl:DatatypeProperty>
  <owl:DatatypeProperty rdf:about="http://example.org/onto/prop/google_access_context_manager_service_perimeters_title">
    <rdfs:label>title</rdfs:label>
    <rdfs:comment>Human readable title. Must be unique within the perimeter. Does not affect behavior.</rdfs:comment>
    <rdfs:domain rdf:resource="http://example.org/onto/class/google_access_context_manager_service_perimeters"/>
    <rdfs:range rdf:resource="http://www.w3.org/2001/XMLSchema#string"/>
  </owl:DatatypeProperty>
  <owl:DatatypeProperty rdf:about="http://example.org/onto/prop/google_access_context_manager_service_perimeters_identities">
    <rdfs:label>identities</rdfs:label>
    <rdfs:comment>A list of identities that are allowed access through this ingress policy.
Should be in the format of email address. The email address should represent
individual user or service account only.</rdfs:comment>
    <rdfs:domain rdf:resource="http://example.org/onto/class/google_access_context_manager_service_perimeters"/>
    <rdfs:range rdf:resource="http://www.w3.org/2001/XMLSchema#string"/>
  </owl:DatatypeProperty>
  <owl:DatatypeProperty rdf:about="http://example.org/onto/prop/google_access_context_manager_service_perimeters_identity_type">
    <rdfs:label>identity_type</rdfs:label>
    <rdfs:comment>Specifies the type of identities that are allowed access from outside the
perimeter. If left unspecified, then members of 'identities' field will be
allowed access. Possible values: ["IDENTITY_TYPE_UNSPECIFIED", "ANY_IDENTITY", "ANY_USER_ACCOUNT", "ANY_SERVICE_ACCOUNT"]</rdfs:comment>
    <rdfs:domain rdf:resource="http://example.org/onto/class/google_access_context_manager_service_perimeters"/>
    <rdfs:range rdf:resource="http://www.w3.org/2001/XMLSchema#string"/>
  </owl:DatatypeProperty>
  <owl:DatatypeProperty rdf:about="http://example.org/onto/prop/google_access_context_manager_service_perimeters_access_level">
    <rdfs:label>access_level</rdfs:label>
    <rdfs:comment>An 'AccessLevel' resource name that allow resources within the
'ServicePerimeters' to be accessed from the internet. 'AccessLevels' listed
must be in the same policy as this 'ServicePerimeter'. Referencing a nonexistent
'AccessLevel' will cause an error. If no 'AccessLevel' names are listed,
resources within the perimeter can only be accessed via Google Cloud calls
with request origins within the perimeter.
Example 'accessPolicies/MY_POLICY/accessLevels/MY_LEVEL.'
If * is specified, then all IngressSources will be allowed.</rdfs:comment>
    <rdfs:domain rdf:resource="http://example.org/onto/class/google_access_context_manager_service_perimeters"/>
    <rdfs:range rdf:resource="http://www.w3.org/2001/XMLSchema#string"/>
  </owl:DatatypeProperty>
  <owl:DatatypeProperty rdf:about="http://example.org/onto/prop/google_access_context_manager_service_perimeters_resource">
    <rdfs:label>resource</rdfs:label>
    <rdfs:comment>A Google Cloud resource that is allowed to ingress the perimeter.
Requests from these resources will be allowed to access perimeter data.
Currently only projects are allowed. Format 'projects/{project_number}'
The project may be in any Google Cloud organization, not just the
organization that the perimeter is defined in. '*' is not allowed, the case
of allowing all Google Cloud resources only is not supported.</rdfs:comment>
    <rdfs:domain rdf:resource="http://example.org/onto/class/google_access_context_manager_service_perimeters"/>
    <rdfs:range rdf:resource="http://www.w3.org/2001/XMLSchema#string"/>
  </owl:DatatypeProperty>
  <owl:DatatypeProperty rdf:about="http://example.org/onto/prop/google_access_context_manager_service_perimeters_resources">
    <rdfs:label>resources</rdfs:label>
    <rdfs:comment>A list of resources, currently only projects in the form
'projects/<projectnumber>', protected by this 'ServicePerimeter'
that are allowed to be accessed by sources defined in the
corresponding 'IngressFrom'. A request matches if it contains
a resource in this list. If '*' is specified for resources,
then this 'IngressTo' rule will authorize access to all
resources inside the perimeter, provided that the request
also matches the 'operations' field.</rdfs:comment>
    <rdfs:domain rdf:resource="http://example.org/onto/class/google_access_context_manager_service_perimeters"/>
    <rdfs:range rdf:resource="http://www.w3.org/2001/XMLSchema#string"/>
  </owl:DatatypeProperty>
  <owl:DatatypeProperty rdf:about="http://example.org/onto/prop/google_access_context_manager_service_perimeters_roles">
    <rdfs:label>roles</rdfs:label>
    <rdfs:comment>A list of IAM roles that represent the set of operations that the sources
specified in the corresponding 'IngressFrom'
are allowed to perform.</rdfs:comment>
    <rdfs:domain rdf:resource="http://example.org/onto/class/google_access_context_manager_service_perimeters"/>
    <rdfs:range rdf:resource="http://www.w3.org/2001/XMLSchema#string"/>
  </owl:DatatypeProperty>
  <owl:DatatypeProperty rdf:about="http://example.org/onto/prop/google_access_context_manager_service_perimeters_service_name">
    <rdfs:label>service_name</rdfs:label>
    <rdfs:comment>The name of the API whose methods or permissions the 'IngressPolicy' or
'EgressPolicy' want to allow. A single 'ApiOperation' with 'serviceName'
field set to '*' will allow all methods AND permissions for all services.</rdfs:comment>
    <rdfs:domain rdf:resource="http://example.org/onto/class/google_access_context_manager_service_perimeters"/>
    <rdfs:range rdf:resource="http://www.w3.org/2001/XMLSchema#string"/>
  </owl:DatatypeProperty>
  <owl:DatatypeProperty rdf:about="http://example.org/onto/prop/google_access_context_manager_service_perimeters_method">
    <rdfs:label>method</rdfs:label>
    <rdfs:comment>Value for method should be a valid method name for the corresponding
serviceName in 'ApiOperation'. If '*' used as value for 'method', then
ALL methods and permissions are allowed.</rdfs:comment>
    <rdfs:domain rdf:resource="http://example.org/onto/class/google_access_context_manager_service_perimeters"/>
    <rdfs:range rdf:resource="http://www.w3.org/2001/XMLSchema#string"/>
  </owl:DatatypeProperty>
  <owl:DatatypeProperty rdf:about="http://example.org/onto/prop/google_access_context_manager_service_perimeters_permission">
    <rdfs:label>permission</rdfs:label>
    <rdfs:comment>Value for permission should be a valid Cloud IAM permission for the
corresponding 'serviceName' in 'ApiOperation'.</rdfs:comment>
    <rdfs:domain rdf:resource="http://example.org/onto/class/google_access_context_manager_service_perimeters"/>
    <rdfs:range rdf:resource="http://www.w3.org/2001/XMLSchema#string"/>
  </owl:DatatypeProperty>
  <owl:DatatypeProperty rdf:about="http://example.org/onto/prop/google_access_context_manager_service_perimeters_allowed_services">
    <rdfs:label>allowed_services</rdfs:label>
    <rdfs:comment>The list of APIs usable within the Service Perimeter.
Must be empty unless 'enableRestriction' is True.</rdfs:comment>
    <rdfs:domain rdf:resource="http://example.org/onto/class/google_access_context_manager_service_perimeters"/>
    <rdfs:range rdf:resource="http://www.w3.org/2001/XMLSchema#string"/>
  </owl:DatatypeProperty>
  <owl:DatatypeProperty rdf:about="http://example.org/onto/prop/google_access_context_manager_service_perimeters_enable_restriction">
    <rdfs:label>enable_restriction</rdfs:label>
    <rdfs:comment>Whether to restrict API calls within the Service Perimeter to the
list of APIs specified in 'allowedServices'.</rdfs:comment>
    <rdfs:domain rdf:resource="http://example.org/onto/class/google_access_context_manager_service_perimeters"/>
    <rdfs:range rdf:resource="http://www.w3.org/2001/XMLSchema#string"/>
  </owl:DatatypeProperty>
  <owl:DatatypeProperty rdf:about="http://example.org/onto/prop/google_access_context_manager_service_perimeters_create">
    <rdfs:label>create</rdfs:label>
    <rdfs:domain rdf:resource="http://example.org/onto/class/google_access_context_manager_service_perimeters"/>
    <rdfs:range rdf:resource="http://www.w3.org/2001/XMLSchema#string"/>
  </owl:DatatypeProperty>
  <owl:DatatypeProperty rdf:about="http://example.org/onto/prop/google_access_context_manager_service_perimeters_delete">
    <rdfs:label>delete</rdfs:label>
    <rdfs:domain rdf:resource="http://example.org/onto/class/google_access_context_manager_service_perimeters"/>
    <rdfs:range rdf:resource="http://www.w3.org/2001/XMLSchema#string"/>
  </owl:DatatypeProperty>
  <owl:DatatypeProperty rdf:about="http://example.org/onto/prop/google_access_context_manager_service_perimeters_update">
    <rdfs:label>update</rdfs:label>
    <rdfs:domain rdf:resource="http://example.org/onto/class/google_access_context_manager_service_perimeters"/>
    <rdfs:range rdf:resource="http://www.w3.org/2001/XMLSchema#string"/>
  </owl:DatatypeProperty>
</rdf:RDF>
