<?xml version="1.0" encoding="UTF-8"?>
<rdf:RDF
  xmlns:rdf="http://www.w3.org/1999/02/22-rdf-syntax-ns#"
  xmlns:rdfs="http://www.w3.org/2000/01/rdf-schema#"
  xmlns:owl="http://www.w3.org/2002/07/owl#"
  xmlns:xsd="http://www.w3.org/2001/XMLSchema#"
  xml:base="http://example.org/onto/">
  <owl:Class rdf:about="http://example.org/onto/class/google_dataproc_workflow_template">
    <rdfs:label>google_dataproc_workflow_template</rdfs:label>
    <rdfs:comment>#
#     ***     AUTO GENERATED CODE    ***    Type: Handwritten     ***
#
# ----------------------------------------------------------------------------
#
#     This code is generated by Magic Modules using the following:
#
#     Source file: https://github.com/GoogleCloudPlatform/magic-modules/tree/main/mmv1/third_party/terraform/website/docs/r/dataproc_workflow_template.html.markdown
#
#     DO NOT EDIT this file directly. Any changes made to this file will be
#     overwritten during the next generation cycle.
#
# ----------------------------------------------------------------------------
subcategory: "Dataproc"
description: |-
  A Workflow Template is a reusable workflow configuration.
---</rdfs:comment>
  </owl:Class>
  <owl:DatatypeProperty rdf:about="http://example.org/onto/prop/google_dataproc_workflow_template_create_time">
    <rdfs:label>create_time</rdfs:label>
    <rdfs:comment>Output only. The time template was created.</rdfs:comment>
    <rdfs:domain rdf:resource="http://example.org/onto/class/google_dataproc_workflow_template"/>
    <rdfs:range rdf:resource="http://www.w3.org/2001/XMLSchema#string"/>
  </owl:DatatypeProperty>
  <owl:DatatypeProperty rdf:about="http://example.org/onto/prop/google_dataproc_workflow_template_dag_timeout">
    <rdfs:label>dag_timeout</rdfs:label>
    <rdfs:comment>Optional. Timeout duration for the DAG of jobs, expressed in seconds (see [JSON representation of duration](https://developers.google.com/protocol-buffers/docs/proto3#json)). The timeout duration must be from 10 minutes ("600s") to 24 hours ("86400s"). The timer begins when the first job is submitted. If the workflow is running at the end of the timeout period, any remaining jobs are cancelled, the workflow is ended, and if the workflow was running on a [managed cluster](/dataproc/docs/concepts/workflows/using-workflows#configuring_or_selecting_a_cluster), the cluster is deleted.</rdfs:comment>
    <rdfs:domain rdf:resource="http://example.org/onto/class/google_dataproc_workflow_template"/>
    <rdfs:range rdf:resource="http://www.w3.org/2001/XMLSchema#string"/>
  </owl:DatatypeProperty>
  <owl:DatatypeProperty rdf:about="http://example.org/onto/prop/google_dataproc_workflow_template_effective_labels">
    <rdfs:label>effective_labels</rdfs:label>
    <rdfs:comment>All of labels (key/value pairs) present on the resource in GCP, including the labels configured through Terraform, other clients and services.</rdfs:comment>
    <rdfs:domain rdf:resource="http://example.org/onto/class/google_dataproc_workflow_template"/>
    <rdfs:range rdf:resource="http://www.w3.org/2001/XMLSchema#string"/>
  </owl:DatatypeProperty>
  <owl:DatatypeProperty rdf:about="http://example.org/onto/prop/google_dataproc_workflow_template_id">
    <rdfs:label>id</rdfs:label>
    <rdfs:domain rdf:resource="http://example.org/onto/class/google_dataproc_workflow_template"/>
    <rdfs:range rdf:resource="http://www.w3.org/2001/XMLSchema#string"/>
  </owl:DatatypeProperty>
  <owl:DatatypeProperty rdf:about="http://example.org/onto/prop/google_dataproc_workflow_template_labels">
    <rdfs:label>labels</rdfs:label>
    <rdfs:comment>Optional. The labels to associate with this template. These labels will be propagated to all jobs and clusters created by the workflow instance. Label **keys** must contain 1 to 63 characters, and must conform to [RFC 1035](https://www.ietf.org/rfc/rfc1035.txt). Label **values** may be empty, but, if present, must contain 1 to 63 characters, and must conform to [RFC 1035](https://www.ietf.org/rfc/rfc1035.txt). No more than 32 labels can be associated with a template.

**Note**: This field is non-authoritative, and will only manage the labels present in your configuration.
Please refer to the field `effective_labels` for all of the labels present on the resource.</rdfs:comment>
    <rdfs:domain rdf:resource="http://example.org/onto/class/google_dataproc_workflow_template"/>
    <rdfs:range rdf:resource="http://www.w3.org/2001/XMLSchema#string"/>
  </owl:DatatypeProperty>
  <owl:DatatypeProperty rdf:about="http://example.org/onto/prop/google_dataproc_workflow_template_location">
    <rdfs:label>location</rdfs:label>
    <rdfs:comment>The location for the resource</rdfs:comment>
    <rdfs:domain rdf:resource="http://example.org/onto/class/google_dataproc_workflow_template"/>
    <rdfs:range rdf:resource="http://www.w3.org/2001/XMLSchema#string"/>
  </owl:DatatypeProperty>
  <owl:DatatypeProperty rdf:about="http://example.org/onto/prop/google_dataproc_workflow_template_name">
    <rdfs:label>name</rdfs:label>
    <rdfs:comment>Output only. The resource name of the workflow template, as described in https://cloud.google.com/apis/design/resource_names. * For `projects.regions.workflowTemplates`, the resource name of the template has the following format: `projects/{project_id}/regions/{region}/workflowTemplates/{template_id}` * For `projects.locations.workflowTemplates`, the resource name of the template has the following format: `projects/{project_id}/locations/{location}/workflowTemplates/{template_id}`</rdfs:comment>
    <rdfs:domain rdf:resource="http://example.org/onto/class/google_dataproc_workflow_template"/>
    <rdfs:range rdf:resource="http://www.w3.org/2001/XMLSchema#string"/>
  </owl:DatatypeProperty>
  <owl:DatatypeProperty rdf:about="http://example.org/onto/prop/google_dataproc_workflow_template_project">
    <rdfs:label>project</rdfs:label>
    <rdfs:comment>The project for the resource</rdfs:comment>
    <rdfs:domain rdf:resource="http://example.org/onto/class/google_dataproc_workflow_template"/>
    <rdfs:range rdf:resource="http://www.w3.org/2001/XMLSchema#string"/>
  </owl:DatatypeProperty>
  <owl:DatatypeProperty rdf:about="http://example.org/onto/prop/google_dataproc_workflow_template_terraform_labels">
    <rdfs:label>terraform_labels</rdfs:label>
    <rdfs:comment>The combination of labels configured directly on the resource and default labels configured on the provider.</rdfs:comment>
    <rdfs:domain rdf:resource="http://example.org/onto/class/google_dataproc_workflow_template"/>
    <rdfs:range rdf:resource="http://www.w3.org/2001/XMLSchema#string"/>
  </owl:DatatypeProperty>
  <owl:DatatypeProperty rdf:about="http://example.org/onto/prop/google_dataproc_workflow_template_update_time">
    <rdfs:label>update_time</rdfs:label>
    <rdfs:comment>Output only. The time template was last updated.</rdfs:comment>
    <rdfs:domain rdf:resource="http://example.org/onto/class/google_dataproc_workflow_template"/>
    <rdfs:range rdf:resource="http://www.w3.org/2001/XMLSchema#string"/>
  </owl:DatatypeProperty>
  <owl:DatatypeProperty rdf:about="http://example.org/onto/prop/google_dataproc_workflow_template_version">
    <rdfs:label>version</rdfs:label>
    <rdfs:comment>Output only. The current version of this workflow template.</rdfs:comment>
    <rdfs:domain rdf:resource="http://example.org/onto/class/google_dataproc_workflow_template"/>
    <rdfs:range rdf:resource="http://www.w3.org/2001/XMLSchema#string"/>
  </owl:DatatypeProperty>
  <owl:DatatypeProperty rdf:about="http://example.org/onto/prop/google_dataproc_workflow_template_kms_key">
    <rdfs:label>kms_key</rdfs:label>
    <rdfs:comment>Optional. The Cloud KMS key name to use for encryption.</rdfs:comment>
    <rdfs:domain rdf:resource="http://example.org/onto/class/google_dataproc_workflow_template"/>
    <rdfs:range rdf:resource="http://www.w3.org/2001/XMLSchema#string"/>
  </owl:DatatypeProperty>
  <owl:DatatypeProperty rdf:about="http://example.org/onto/prop/google_dataproc_workflow_template_labels">
    <rdfs:label>labels</rdfs:label>
    <rdfs:comment>Optional. The labels to associate with this job. Label keys must be between 1 and 63 characters long, and must conform to the following regular expression: p{Ll}p{Lo}{0,62} Label values must be between 1 and 63 characters long, and must conform to the following regular expression: [p{Ll}p{Lo}p{N}_-]{0,63} No more than 32 labels can be associated with a given job.</rdfs:comment>
    <rdfs:domain rdf:resource="http://example.org/onto/class/google_dataproc_workflow_template"/>
    <rdfs:range rdf:resource="http://www.w3.org/2001/XMLSchema#string"/>
  </owl:DatatypeProperty>
  <owl:DatatypeProperty rdf:about="http://example.org/onto/prop/google_dataproc_workflow_template_prerequisite_step_ids">
    <rdfs:label>prerequisite_step_ids</rdfs:label>
    <rdfs:comment>Optional. The optional list of prerequisite job step_ids. If not specified, the job will start at the beginning of workflow.</rdfs:comment>
    <rdfs:domain rdf:resource="http://example.org/onto/class/google_dataproc_workflow_template"/>
    <rdfs:range rdf:resource="http://www.w3.org/2001/XMLSchema#string"/>
  </owl:DatatypeProperty>
  <owl:DatatypeProperty rdf:about="http://example.org/onto/prop/google_dataproc_workflow_template_step_id">
    <rdfs:label>step_id</rdfs:label>
    <rdfs:comment>Required. The step id. The id must be unique among all jobs within the template. The step id is used as prefix for job id, as job `goog-dataproc-workflow-step-id` label, and in prerequisiteStepIds field from other steps. The id must contain only letters (a-z, A-Z), numbers (0-9), underscores (_), and hyphens (-). Cannot begin or end with underscore or hyphen. Must consist of between 3 and 50 characters.</rdfs:comment>
    <rdfs:domain rdf:resource="http://example.org/onto/class/google_dataproc_workflow_template"/>
    <rdfs:range rdf:resource="http://www.w3.org/2001/XMLSchema#string"/>
  </owl:DatatypeProperty>
  <owl:DatatypeProperty rdf:about="http://example.org/onto/prop/google_dataproc_workflow_template_archive_uris">
    <rdfs:label>archive_uris</rdfs:label>
    <rdfs:comment>Optional. HCFS URIs of archives to be extracted in the working directory of Hadoop drivers and tasks. Supported file types: .jar, .tar, .tar.gz, .tgz, or .zip.</rdfs:comment>
    <rdfs:domain rdf:resource="http://example.org/onto/class/google_dataproc_workflow_template"/>
    <rdfs:range rdf:resource="http://www.w3.org/2001/XMLSchema#string"/>
  </owl:DatatypeProperty>
  <owl:DatatypeProperty rdf:about="http://example.org/onto/prop/google_dataproc_workflow_template_args">
    <rdfs:label>args</rdfs:label>
    <rdfs:comment>Optional. The arguments to pass to the driver. Do not include arguments, such as `-libjars` or `-Dfoo=bar`, that can be set as job properties, since a collision may occur that causes an incorrect job submission.</rdfs:comment>
    <rdfs:domain rdf:resource="http://example.org/onto/class/google_dataproc_workflow_template"/>
    <rdfs:range rdf:resource="http://www.w3.org/2001/XMLSchema#string"/>
  </owl:DatatypeProperty>
  <owl:DatatypeProperty rdf:about="http://example.org/onto/prop/google_dataproc_workflow_template_file_uris">
    <rdfs:label>file_uris</rdfs:label>
    <rdfs:comment>Optional. HCFS (Hadoop Compatible Filesystem) URIs of files to be copied to the working directory of Hadoop drivers and distributed tasks. Useful for naively parallel tasks.</rdfs:comment>
    <rdfs:domain rdf:resource="http://example.org/onto/class/google_dataproc_workflow_template"/>
    <rdfs:range rdf:resource="http://www.w3.org/2001/XMLSchema#string"/>
  </owl:DatatypeProperty>
  <owl:DatatypeProperty rdf:about="http://example.org/onto/prop/google_dataproc_workflow_template_jar_file_uris">
    <rdfs:label>jar_file_uris</rdfs:label>
    <rdfs:comment>Optional. Jar file URIs to add to the CLASSPATHs of the Hadoop driver and tasks.</rdfs:comment>
    <rdfs:domain rdf:resource="http://example.org/onto/class/google_dataproc_workflow_template"/>
    <rdfs:range rdf:resource="http://www.w3.org/2001/XMLSchema#string"/>
  </owl:DatatypeProperty>
  <owl:DatatypeProperty rdf:about="http://example.org/onto/prop/google_dataproc_workflow_template_main_class">
    <rdfs:label>main_class</rdfs:label>
    <rdfs:comment>The name of the driver's main class. The jar file containing the class must be in the default CLASSPATH or specified in `jar_file_uris`.</rdfs:comment>
    <rdfs:domain rdf:resource="http://example.org/onto/class/google_dataproc_workflow_template"/>
    <rdfs:range rdf:resource="http://www.w3.org/2001/XMLSchema#string"/>
  </owl:DatatypeProperty>
  <owl:DatatypeProperty rdf:about="http://example.org/onto/prop/google_dataproc_workflow_template_main_jar_file_uri">
    <rdfs:label>main_jar_file_uri</rdfs:label>
    <rdfs:comment>The HCFS URI of the jar file containing the main class. Examples: 'gs://foo-bucket/analytics-binaries/extract-useful-metrics-mr.jar' 'hdfs:/tmp/test-samples/custom-wordcount.jar' 'file:///home/usr/lib/hadoop-mapreduce/hadoop-mapreduce-examples.jar'</rdfs:comment>
    <rdfs:domain rdf:resource="http://example.org/onto/class/google_dataproc_workflow_template"/>
    <rdfs:range rdf:resource="http://www.w3.org/2001/XMLSchema#string"/>
  </owl:DatatypeProperty>
  <owl:DatatypeProperty rdf:about="http://example.org/onto/prop/google_dataproc_workflow_template_properties">
    <rdfs:label>properties</rdfs:label>
    <rdfs:comment>Optional. A mapping of property names to values, used to configure Hadoop. Properties that conflict with values set by the Dataproc API may be overwritten. Can include properties set in /etc/hadoop/conf/*-site and classes in user code.</rdfs:comment>
    <rdfs:domain rdf:resource="http://example.org/onto/class/google_dataproc_workflow_template"/>
    <rdfs:range rdf:resource="http://www.w3.org/2001/XMLSchema#string"/>
  </owl:DatatypeProperty>
  <owl:DatatypeProperty rdf:about="http://example.org/onto/prop/google_dataproc_workflow_template_driver_log_levels">
    <rdfs:label>driver_log_levels</rdfs:label>
    <rdfs:comment>The per-package log levels for the driver. This may include "root" package name to configure rootLogger. Examples: 'com.google = FATAL', 'root = INFO', 'org.apache = DEBUG'</rdfs:comment>
    <rdfs:domain rdf:resource="http://example.org/onto/class/google_dataproc_workflow_template"/>
    <rdfs:range rdf:resource="http://www.w3.org/2001/XMLSchema#string"/>
  </owl:DatatypeProperty>
  <owl:DatatypeProperty rdf:about="http://example.org/onto/prop/google_dataproc_workflow_template_continue_on_failure">
    <rdfs:label>continue_on_failure</rdfs:label>
    <rdfs:comment>Optional. Whether to continue executing queries if a query fails. The default value is `false`. Setting to `true` can be useful when executing independent parallel queries.</rdfs:comment>
    <rdfs:domain rdf:resource="http://example.org/onto/class/google_dataproc_workflow_template"/>
    <rdfs:range rdf:resource="http://www.w3.org/2001/XMLSchema#string"/>
  </owl:DatatypeProperty>
  <owl:DatatypeProperty rdf:about="http://example.org/onto/prop/google_dataproc_workflow_template_jar_file_uris">
    <rdfs:label>jar_file_uris</rdfs:label>
    <rdfs:comment>Optional. HCFS URIs of jar files to add to the CLASSPATH of the Hive server and Hadoop MapReduce (MR) tasks. Can contain Hive SerDes and UDFs.</rdfs:comment>
    <rdfs:domain rdf:resource="http://example.org/onto/class/google_dataproc_workflow_template"/>
    <rdfs:range rdf:resource="http://www.w3.org/2001/XMLSchema#string"/>
  </owl:DatatypeProperty>
  <owl:DatatypeProperty rdf:about="http://example.org/onto/prop/google_dataproc_workflow_template_properties">
    <rdfs:label>properties</rdfs:label>
    <rdfs:comment>Optional. A mapping of property names and values, used to configure Hive. Properties that conflict with values set by the Dataproc API may be overwritten. Can include properties set in /etc/hadoop/conf/*-site.xml, /etc/hive/conf/hive-site.xml, and classes in user code.</rdfs:comment>
    <rdfs:domain rdf:resource="http://example.org/onto/class/google_dataproc_workflow_template"/>
    <rdfs:range rdf:resource="http://www.w3.org/2001/XMLSchema#string"/>
  </owl:DatatypeProperty>
  <owl:DatatypeProperty rdf:about="http://example.org/onto/prop/google_dataproc_workflow_template_query_file_uri">
    <rdfs:label>query_file_uri</rdfs:label>
    <rdfs:comment>The HCFS URI of the script that contains Hive queries.</rdfs:comment>
    <rdfs:domain rdf:resource="http://example.org/onto/class/google_dataproc_workflow_template"/>
    <rdfs:range rdf:resource="http://www.w3.org/2001/XMLSchema#string"/>
  </owl:DatatypeProperty>
  <owl:DatatypeProperty rdf:about="http://example.org/onto/prop/google_dataproc_workflow_template_script_variables">
    <rdfs:label>script_variables</rdfs:label>
    <rdfs:comment>Optional. Mapping of query variable names to values (equivalent to the Hive command: `SET name="value";`).</rdfs:comment>
    <rdfs:domain rdf:resource="http://example.org/onto/class/google_dataproc_workflow_template"/>
    <rdfs:range rdf:resource="http://www.w3.org/2001/XMLSchema#string"/>
  </owl:DatatypeProperty>
  <owl:DatatypeProperty rdf:about="http://example.org/onto/prop/google_dataproc_workflow_template_queries">
    <rdfs:label>queries</rdfs:label>
    <rdfs:comment>Required. The queries to execute. You do not need to end a query expression with a semicolon. Multiple queries can be specified in one string by separating each with a semicolon. Here is an example of a Dataproc API snippet that uses a QueryList to specify a HiveJob: "hiveJob": { "queryList": { "queries": [ "query1", "query2", "query3;query4", ] } }</rdfs:comment>
    <rdfs:domain rdf:resource="http://example.org/onto/class/google_dataproc_workflow_template"/>
    <rdfs:range rdf:resource="http://www.w3.org/2001/XMLSchema#string"/>
  </owl:DatatypeProperty>
  <owl:DatatypeProperty rdf:about="http://example.org/onto/prop/google_dataproc_workflow_template_continue_on_failure">
    <rdfs:label>continue_on_failure</rdfs:label>
    <rdfs:comment>Optional. Whether to continue executing queries if a query fails. The default value is `false`. Setting to `true` can be useful when executing independent parallel queries.</rdfs:comment>
    <rdfs:domain rdf:resource="http://example.org/onto/class/google_dataproc_workflow_template"/>
    <rdfs:range rdf:resource="http://www.w3.org/2001/XMLSchema#string"/>
  </owl:DatatypeProperty>
  <owl:DatatypeProperty rdf:about="http://example.org/onto/prop/google_dataproc_workflow_template_jar_file_uris">
    <rdfs:label>jar_file_uris</rdfs:label>
    <rdfs:comment>Optional. HCFS URIs of jar files to add to the CLASSPATH of the Pig Client and Hadoop MapReduce (MR) tasks. Can contain Pig UDFs.</rdfs:comment>
    <rdfs:domain rdf:resource="http://example.org/onto/class/google_dataproc_workflow_template"/>
    <rdfs:range rdf:resource="http://www.w3.org/2001/XMLSchema#string"/>
  </owl:DatatypeProperty>
  <owl:DatatypeProperty rdf:about="http://example.org/onto/prop/google_dataproc_workflow_template_properties">
    <rdfs:label>properties</rdfs:label>
    <rdfs:comment>Optional. A mapping of property names to values, used to configure Pig. Properties that conflict with values set by the Dataproc API may be overwritten. Can include properties set in /etc/hadoop/conf/*-site.xml, /etc/pig/conf/pig.properties, and classes in user code.</rdfs:comment>
    <rdfs:domain rdf:resource="http://example.org/onto/class/google_dataproc_workflow_template"/>
    <rdfs:range rdf:resource="http://www.w3.org/2001/XMLSchema#string"/>
  </owl:DatatypeProperty>
  <owl:DatatypeProperty rdf:about="http://example.org/onto/prop/google_dataproc_workflow_template_query_file_uri">
    <rdfs:label>query_file_uri</rdfs:label>
    <rdfs:comment>The HCFS URI of the script that contains the Pig queries.</rdfs:comment>
    <rdfs:domain rdf:resource="http://example.org/onto/class/google_dataproc_workflow_template"/>
    <rdfs:range rdf:resource="http://www.w3.org/2001/XMLSchema#string"/>
  </owl:DatatypeProperty>
  <owl:DatatypeProperty rdf:about="http://example.org/onto/prop/google_dataproc_workflow_template_script_variables">
    <rdfs:label>script_variables</rdfs:label>
    <rdfs:comment>Optional. Mapping of query variable names to values (equivalent to the Pig command: `name=[value]`).</rdfs:comment>
    <rdfs:domain rdf:resource="http://example.org/onto/class/google_dataproc_workflow_template"/>
    <rdfs:range rdf:resource="http://www.w3.org/2001/XMLSchema#string"/>
  </owl:DatatypeProperty>
  <owl:DatatypeProperty rdf:about="http://example.org/onto/prop/google_dataproc_workflow_template_driver_log_levels">
    <rdfs:label>driver_log_levels</rdfs:label>
    <rdfs:comment>The per-package log levels for the driver. This may include "root" package name to configure rootLogger. Examples: 'com.google = FATAL', 'root = INFO', 'org.apache = DEBUG'</rdfs:comment>
    <rdfs:domain rdf:resource="http://example.org/onto/class/google_dataproc_workflow_template"/>
    <rdfs:range rdf:resource="http://www.w3.org/2001/XMLSchema#string"/>
  </owl:DatatypeProperty>
  <owl:DatatypeProperty rdf:about="http://example.org/onto/prop/google_dataproc_workflow_template_queries">
    <rdfs:label>queries</rdfs:label>
    <rdfs:comment>Required. The queries to execute. You do not need to end a query expression with a semicolon. Multiple queries can be specified in one string by separating each with a semicolon. Here is an example of a Dataproc API snippet that uses a QueryList to specify a HiveJob: "hiveJob": { "queryList": { "queries": [ "query1", "query2", "query3;query4", ] } }</rdfs:comment>
    <rdfs:domain rdf:resource="http://example.org/onto/class/google_dataproc_workflow_template"/>
    <rdfs:range rdf:resource="http://www.w3.org/2001/XMLSchema#string"/>
  </owl:DatatypeProperty>
  <owl:DatatypeProperty rdf:about="http://example.org/onto/prop/google_dataproc_workflow_template_client_tags">
    <rdfs:label>client_tags</rdfs:label>
    <rdfs:comment>Optional. Presto client tags to attach to this query</rdfs:comment>
    <rdfs:domain rdf:resource="http://example.org/onto/class/google_dataproc_workflow_template"/>
    <rdfs:range rdf:resource="http://www.w3.org/2001/XMLSchema#string"/>
  </owl:DatatypeProperty>
  <owl:DatatypeProperty rdf:about="http://example.org/onto/prop/google_dataproc_workflow_template_continue_on_failure">
    <rdfs:label>continue_on_failure</rdfs:label>
    <rdfs:comment>Optional. Whether to continue executing queries if a query fails. The default value is `false`. Setting to `true` can be useful when executing independent parallel queries.</rdfs:comment>
    <rdfs:domain rdf:resource="http://example.org/onto/class/google_dataproc_workflow_template"/>
    <rdfs:range rdf:resource="http://www.w3.org/2001/XMLSchema#string"/>
  </owl:DatatypeProperty>
  <owl:DatatypeProperty rdf:about="http://example.org/onto/prop/google_dataproc_workflow_template_output_format">
    <rdfs:label>output_format</rdfs:label>
    <rdfs:comment>Optional. The format in which query output will be displayed. See the Presto documentation for supported output formats</rdfs:comment>
    <rdfs:domain rdf:resource="http://example.org/onto/class/google_dataproc_workflow_template"/>
    <rdfs:range rdf:resource="http://www.w3.org/2001/XMLSchema#string"/>
  </owl:DatatypeProperty>
  <owl:DatatypeProperty rdf:about="http://example.org/onto/prop/google_dataproc_workflow_template_properties">
    <rdfs:label>properties</rdfs:label>
    <rdfs:comment>Optional. A mapping of property names to values. Used to set Presto [session properties](https://prestodb.io/docs/current/sql/set-session.html) Equivalent to using the --session flag in the Presto CLI</rdfs:comment>
    <rdfs:domain rdf:resource="http://example.org/onto/class/google_dataproc_workflow_template"/>
    <rdfs:range rdf:resource="http://www.w3.org/2001/XMLSchema#string"/>
  </owl:DatatypeProperty>
  <owl:DatatypeProperty rdf:about="http://example.org/onto/prop/google_dataproc_workflow_template_query_file_uri">
    <rdfs:label>query_file_uri</rdfs:label>
    <rdfs:comment>The HCFS URI of the script that contains SQL queries.</rdfs:comment>
    <rdfs:domain rdf:resource="http://example.org/onto/class/google_dataproc_workflow_template"/>
    <rdfs:range rdf:resource="http://www.w3.org/2001/XMLSchema#string"/>
  </owl:DatatypeProperty>
  <owl:DatatypeProperty rdf:about="http://example.org/onto/prop/google_dataproc_workflow_template_driver_log_levels">
    <rdfs:label>driver_log_levels</rdfs:label>
    <rdfs:comment>The per-package log levels for the driver. This may include "root" package name to configure rootLogger. Examples: 'com.google = FATAL', 'root = INFO', 'org.apache = DEBUG'</rdfs:comment>
    <rdfs:domain rdf:resource="http://example.org/onto/class/google_dataproc_workflow_template"/>
    <rdfs:range rdf:resource="http://www.w3.org/2001/XMLSchema#string"/>
  </owl:DatatypeProperty>
  <owl:DatatypeProperty rdf:about="http://example.org/onto/prop/google_dataproc_workflow_template_queries">
    <rdfs:label>queries</rdfs:label>
    <rdfs:comment>Required. The queries to execute. You do not need to end a query expression with a semicolon. Multiple queries can be specified in one string by separating each with a semicolon. Here is an example of a Dataproc API snippet that uses a QueryList to specify a HiveJob: "hiveJob": { "queryList": { "queries": [ "query1", "query2", "query3;query4", ] } }</rdfs:comment>
    <rdfs:domain rdf:resource="http://example.org/onto/class/google_dataproc_workflow_template"/>
    <rdfs:range rdf:resource="http://www.w3.org/2001/XMLSchema#string"/>
  </owl:DatatypeProperty>
  <owl:DatatypeProperty rdf:about="http://example.org/onto/prop/google_dataproc_workflow_template_archive_uris">
    <rdfs:label>archive_uris</rdfs:label>
    <rdfs:comment>Optional. HCFS URIs of archives to be extracted into the working directory of each executor. Supported file types: .jar, .tar, .tar.gz, .tgz, and .zip.</rdfs:comment>
    <rdfs:domain rdf:resource="http://example.org/onto/class/google_dataproc_workflow_template"/>
    <rdfs:range rdf:resource="http://www.w3.org/2001/XMLSchema#string"/>
  </owl:DatatypeProperty>
  <owl:DatatypeProperty rdf:about="http://example.org/onto/prop/google_dataproc_workflow_template_args">
    <rdfs:label>args</rdfs:label>
    <rdfs:comment>Optional. The arguments to pass to the driver. Do not include arguments, such as `--conf`, that can be set as job properties, since a collision may occur that causes an incorrect job submission.</rdfs:comment>
    <rdfs:domain rdf:resource="http://example.org/onto/class/google_dataproc_workflow_template"/>
    <rdfs:range rdf:resource="http://www.w3.org/2001/XMLSchema#string"/>
  </owl:DatatypeProperty>
  <owl:DatatypeProperty rdf:about="http://example.org/onto/prop/google_dataproc_workflow_template_file_uris">
    <rdfs:label>file_uris</rdfs:label>
    <rdfs:comment>Optional. HCFS URIs of files to be placed in the working directory of each executor. Useful for naively parallel tasks.</rdfs:comment>
    <rdfs:domain rdf:resource="http://example.org/onto/class/google_dataproc_workflow_template"/>
    <rdfs:range rdf:resource="http://www.w3.org/2001/XMLSchema#string"/>
  </owl:DatatypeProperty>
  <owl:DatatypeProperty rdf:about="http://example.org/onto/prop/google_dataproc_workflow_template_jar_file_uris">
    <rdfs:label>jar_file_uris</rdfs:label>
    <rdfs:comment>Optional. HCFS URIs of jar files to add to the CLASSPATHs of the Python driver and tasks.</rdfs:comment>
    <rdfs:domain rdf:resource="http://example.org/onto/class/google_dataproc_workflow_template"/>
    <rdfs:range rdf:resource="http://www.w3.org/2001/XMLSchema#string"/>
  </owl:DatatypeProperty>
  <owl:DatatypeProperty rdf:about="http://example.org/onto/prop/google_dataproc_workflow_template_main_python_file_uri">
    <rdfs:label>main_python_file_uri</rdfs:label>
    <rdfs:comment>Required. The HCFS URI of the main Python file to use as the driver. Must be a .py file.</rdfs:comment>
    <rdfs:domain rdf:resource="http://example.org/onto/class/google_dataproc_workflow_template"/>
    <rdfs:range rdf:resource="http://www.w3.org/2001/XMLSchema#string"/>
  </owl:DatatypeProperty>
  <owl:DatatypeProperty rdf:about="http://example.org/onto/prop/google_dataproc_workflow_template_properties">
    <rdfs:label>properties</rdfs:label>
    <rdfs:comment>Optional. A mapping of property names to values, used to configure PySpark. Properties that conflict with values set by the Dataproc API may be overwritten. Can include properties set in /etc/spark/conf/spark-defaults.conf and classes in user code.</rdfs:comment>
    <rdfs:domain rdf:resource="http://example.org/onto/class/google_dataproc_workflow_template"/>
    <rdfs:range rdf:resource="http://www.w3.org/2001/XMLSchema#string"/>
  </owl:DatatypeProperty>
  <owl:DatatypeProperty rdf:about="http://example.org/onto/prop/google_dataproc_workflow_template_python_file_uris">
    <rdfs:label>python_file_uris</rdfs:label>
    <rdfs:comment>Optional. HCFS file URIs of Python files to pass to the PySpark framework. Supported file types: .py, .egg, and .zip.</rdfs:comment>
    <rdfs:domain rdf:resource="http://example.org/onto/class/google_dataproc_workflow_template"/>
    <rdfs:range rdf:resource="http://www.w3.org/2001/XMLSchema#string"/>
  </owl:DatatypeProperty>
  <owl:DatatypeProperty rdf:about="http://example.org/onto/prop/google_dataproc_workflow_template_driver_log_levels">
    <rdfs:label>driver_log_levels</rdfs:label>
    <rdfs:comment>The per-package log levels for the driver. This may include "root" package name to configure rootLogger. Examples: 'com.google = FATAL', 'root = INFO', 'org.apache = DEBUG'</rdfs:comment>
    <rdfs:domain rdf:resource="http://example.org/onto/class/google_dataproc_workflow_template"/>
    <rdfs:range rdf:resource="http://www.w3.org/2001/XMLSchema#string"/>
  </owl:DatatypeProperty>
  <owl:DatatypeProperty rdf:about="http://example.org/onto/prop/google_dataproc_workflow_template_max_failures_per_hour">
    <rdfs:label>max_failures_per_hour</rdfs:label>
    <rdfs:comment>Optional. Maximum number of times per hour a driver may be restarted as a result of driver exiting with non-zero code before job is reported failed. A job may be reported as thrashing if driver exits with non-zero code 4 times within 10 minute window. Maximum value is 10.</rdfs:comment>
    <rdfs:domain rdf:resource="http://example.org/onto/class/google_dataproc_workflow_template"/>
    <rdfs:range rdf:resource="http://www.w3.org/2001/XMLSchema#string"/>
  </owl:DatatypeProperty>
  <owl:DatatypeProperty rdf:about="http://example.org/onto/prop/google_dataproc_workflow_template_max_failures_total">
    <rdfs:label>max_failures_total</rdfs:label>
    <rdfs:comment>Optional. Maximum number of times in total a driver may be restarted as a result of driver exiting with non-zero code before job is reported failed. Maximum value is 240.</rdfs:comment>
    <rdfs:domain rdf:resource="http://example.org/onto/class/google_dataproc_workflow_template"/>
    <rdfs:range rdf:resource="http://www.w3.org/2001/XMLSchema#string"/>
  </owl:DatatypeProperty>
  <owl:DatatypeProperty rdf:about="http://example.org/onto/prop/google_dataproc_workflow_template_archive_uris">
    <rdfs:label>archive_uris</rdfs:label>
    <rdfs:comment>Optional. HCFS URIs of archives to be extracted into the working directory of each executor. Supported file types: .jar, .tar, .tar.gz, .tgz, and .zip.</rdfs:comment>
    <rdfs:domain rdf:resource="http://example.org/onto/class/google_dataproc_workflow_template"/>
    <rdfs:range rdf:resource="http://www.w3.org/2001/XMLSchema#string"/>
  </owl:DatatypeProperty>
  <owl:DatatypeProperty rdf:about="http://example.org/onto/prop/google_dataproc_workflow_template_args">
    <rdfs:label>args</rdfs:label>
    <rdfs:comment>Optional. The arguments to pass to the driver. Do not include arguments, such as `--conf`, that can be set as job properties, since a collision may occur that causes an incorrect job submission.</rdfs:comment>
    <rdfs:domain rdf:resource="http://example.org/onto/class/google_dataproc_workflow_template"/>
    <rdfs:range rdf:resource="http://www.w3.org/2001/XMLSchema#string"/>
  </owl:DatatypeProperty>
  <owl:DatatypeProperty rdf:about="http://example.org/onto/prop/google_dataproc_workflow_template_file_uris">
    <rdfs:label>file_uris</rdfs:label>
    <rdfs:comment>Optional. HCFS URIs of files to be placed in the working directory of each executor. Useful for naively parallel tasks.</rdfs:comment>
    <rdfs:domain rdf:resource="http://example.org/onto/class/google_dataproc_workflow_template"/>
    <rdfs:range rdf:resource="http://www.w3.org/2001/XMLSchema#string"/>
  </owl:DatatypeProperty>
  <owl:DatatypeProperty rdf:about="http://example.org/onto/prop/google_dataproc_workflow_template_jar_file_uris">
    <rdfs:label>jar_file_uris</rdfs:label>
    <rdfs:comment>Optional. HCFS URIs of jar files to add to the CLASSPATHs of the Spark driver and tasks.</rdfs:comment>
    <rdfs:domain rdf:resource="http://example.org/onto/class/google_dataproc_workflow_template"/>
    <rdfs:range rdf:resource="http://www.w3.org/2001/XMLSchema#string"/>
  </owl:DatatypeProperty>
  <owl:DatatypeProperty rdf:about="http://example.org/onto/prop/google_dataproc_workflow_template_main_class">
    <rdfs:label>main_class</rdfs:label>
    <rdfs:comment>The name of the driver's main class. The jar file that contains the class must be in the default CLASSPATH or specified in `jar_file_uris`.</rdfs:comment>
    <rdfs:domain rdf:resource="http://example.org/onto/class/google_dataproc_workflow_template"/>
    <rdfs:range rdf:resource="http://www.w3.org/2001/XMLSchema#string"/>
  </owl:DatatypeProperty>
  <owl:DatatypeProperty rdf:about="http://example.org/onto/prop/google_dataproc_workflow_template_main_jar_file_uri">
    <rdfs:label>main_jar_file_uri</rdfs:label>
    <rdfs:comment>The HCFS URI of the jar file that contains the main class.</rdfs:comment>
    <rdfs:domain rdf:resource="http://example.org/onto/class/google_dataproc_workflow_template"/>
    <rdfs:range rdf:resource="http://www.w3.org/2001/XMLSchema#string"/>
  </owl:DatatypeProperty>
  <owl:DatatypeProperty rdf:about="http://example.org/onto/prop/google_dataproc_workflow_template_properties">
    <rdfs:label>properties</rdfs:label>
    <rdfs:comment>Optional. A mapping of property names to values, used to configure Spark. Properties that conflict with values set by the Dataproc API may be overwritten. Can include properties set in /etc/spark/conf/spark-defaults.conf and classes in user code.</rdfs:comment>
    <rdfs:domain rdf:resource="http://example.org/onto/class/google_dataproc_workflow_template"/>
    <rdfs:range rdf:resource="http://www.w3.org/2001/XMLSchema#string"/>
  </owl:DatatypeProperty>
  <owl:DatatypeProperty rdf:about="http://example.org/onto/prop/google_dataproc_workflow_template_driver_log_levels">
    <rdfs:label>driver_log_levels</rdfs:label>
    <rdfs:comment>The per-package log levels for the driver. This may include "root" package name to configure rootLogger. Examples: 'com.google = FATAL', 'root = INFO', 'org.apache = DEBUG'</rdfs:comment>
    <rdfs:domain rdf:resource="http://example.org/onto/class/google_dataproc_workflow_template"/>
    <rdfs:range rdf:resource="http://www.w3.org/2001/XMLSchema#string"/>
  </owl:DatatypeProperty>
  <owl:DatatypeProperty rdf:about="http://example.org/onto/prop/google_dataproc_workflow_template_archive_uris">
    <rdfs:label>archive_uris</rdfs:label>
    <rdfs:comment>Optional. HCFS URIs of archives to be extracted into the working directory of each executor. Supported file types: .jar, .tar, .tar.gz, .tgz, and .zip.</rdfs:comment>
    <rdfs:domain rdf:resource="http://example.org/onto/class/google_dataproc_workflow_template"/>
    <rdfs:range rdf:resource="http://www.w3.org/2001/XMLSchema#string"/>
  </owl:DatatypeProperty>
  <owl:DatatypeProperty rdf:about="http://example.org/onto/prop/google_dataproc_workflow_template_args">
    <rdfs:label>args</rdfs:label>
    <rdfs:comment>Optional. The arguments to pass to the driver. Do not include arguments, such as `--conf`, that can be set as job properties, since a collision may occur that causes an incorrect job submission.</rdfs:comment>
    <rdfs:domain rdf:resource="http://example.org/onto/class/google_dataproc_workflow_template"/>
    <rdfs:range rdf:resource="http://www.w3.org/2001/XMLSchema#string"/>
  </owl:DatatypeProperty>
  <owl:DatatypeProperty rdf:about="http://example.org/onto/prop/google_dataproc_workflow_template_file_uris">
    <rdfs:label>file_uris</rdfs:label>
    <rdfs:comment>Optional. HCFS URIs of files to be placed in the working directory of each executor. Useful for naively parallel tasks.</rdfs:comment>
    <rdfs:domain rdf:resource="http://example.org/onto/class/google_dataproc_workflow_template"/>
    <rdfs:range rdf:resource="http://www.w3.org/2001/XMLSchema#string"/>
  </owl:DatatypeProperty>
  <owl:DatatypeProperty rdf:about="http://example.org/onto/prop/google_dataproc_workflow_template_main_r_file_uri">
    <rdfs:label>main_r_file_uri</rdfs:label>
    <rdfs:comment>Required. The HCFS URI of the main R file to use as the driver. Must be a .R file.</rdfs:comment>
    <rdfs:domain rdf:resource="http://example.org/onto/class/google_dataproc_workflow_template"/>
    <rdfs:range rdf:resource="http://www.w3.org/2001/XMLSchema#string"/>
  </owl:DatatypeProperty>
  <owl:DatatypeProperty rdf:about="http://example.org/onto/prop/google_dataproc_workflow_template_properties">
    <rdfs:label>properties</rdfs:label>
    <rdfs:comment>Optional. A mapping of property names to values, used to configure SparkR. Properties that conflict with values set by the Dataproc API may be overwritten. Can include properties set in /etc/spark/conf/spark-defaults.conf and classes in user code.</rdfs:comment>
    <rdfs:domain rdf:resource="http://example.org/onto/class/google_dataproc_workflow_template"/>
    <rdfs:range rdf:resource="http://www.w3.org/2001/XMLSchema#string"/>
  </owl:DatatypeProperty>
  <owl:DatatypeProperty rdf:about="http://example.org/onto/prop/google_dataproc_workflow_template_driver_log_levels">
    <rdfs:label>driver_log_levels</rdfs:label>
    <rdfs:comment>The per-package log levels for the driver. This may include "root" package name to configure rootLogger. Examples: 'com.google = FATAL', 'root = INFO', 'org.apache = DEBUG'</rdfs:comment>
    <rdfs:domain rdf:resource="http://example.org/onto/class/google_dataproc_workflow_template"/>
    <rdfs:range rdf:resource="http://www.w3.org/2001/XMLSchema#string"/>
  </owl:DatatypeProperty>
  <owl:DatatypeProperty rdf:about="http://example.org/onto/prop/google_dataproc_workflow_template_jar_file_uris">
    <rdfs:label>jar_file_uris</rdfs:label>
    <rdfs:comment>Optional. HCFS URIs of jar files to be added to the Spark CLASSPATH.</rdfs:comment>
    <rdfs:domain rdf:resource="http://example.org/onto/class/google_dataproc_workflow_template"/>
    <rdfs:range rdf:resource="http://www.w3.org/2001/XMLSchema#string"/>
  </owl:DatatypeProperty>
  <owl:DatatypeProperty rdf:about="http://example.org/onto/prop/google_dataproc_workflow_template_properties">
    <rdfs:label>properties</rdfs:label>
    <rdfs:comment>Optional. A mapping of property names to values, used to configure Spark SQL's SparkConf. Properties that conflict with values set by the Dataproc API may be overwritten.</rdfs:comment>
    <rdfs:domain rdf:resource="http://example.org/onto/class/google_dataproc_workflow_template"/>
    <rdfs:range rdf:resource="http://www.w3.org/2001/XMLSchema#string"/>
  </owl:DatatypeProperty>
  <owl:DatatypeProperty rdf:about="http://example.org/onto/prop/google_dataproc_workflow_template_query_file_uri">
    <rdfs:label>query_file_uri</rdfs:label>
    <rdfs:comment>The HCFS URI of the script that contains SQL queries.</rdfs:comment>
    <rdfs:domain rdf:resource="http://example.org/onto/class/google_dataproc_workflow_template"/>
    <rdfs:range rdf:resource="http://www.w3.org/2001/XMLSchema#string"/>
  </owl:DatatypeProperty>
  <owl:DatatypeProperty rdf:about="http://example.org/onto/prop/google_dataproc_workflow_template_script_variables">
    <rdfs:label>script_variables</rdfs:label>
    <rdfs:comment>Optional. Mapping of query variable names to values (equivalent to the Spark SQL command: SET `name="value";`).</rdfs:comment>
    <rdfs:domain rdf:resource="http://example.org/onto/class/google_dataproc_workflow_template"/>
    <rdfs:range rdf:resource="http://www.w3.org/2001/XMLSchema#string"/>
  </owl:DatatypeProperty>
  <owl:DatatypeProperty rdf:about="http://example.org/onto/prop/google_dataproc_workflow_template_driver_log_levels">
    <rdfs:label>driver_log_levels</rdfs:label>
    <rdfs:comment>The per-package log levels for the driver. This may include "root" package name to configure rootLogger. Examples: 'com.google = FATAL', 'root = INFO', 'org.apache = DEBUG'</rdfs:comment>
    <rdfs:domain rdf:resource="http://example.org/onto/class/google_dataproc_workflow_template"/>
    <rdfs:range rdf:resource="http://www.w3.org/2001/XMLSchema#string"/>
  </owl:DatatypeProperty>
  <owl:DatatypeProperty rdf:about="http://example.org/onto/prop/google_dataproc_workflow_template_queries">
    <rdfs:label>queries</rdfs:label>
    <rdfs:comment>Required. The queries to execute. You do not need to end a query expression with a semicolon. Multiple queries can be specified in one string by separating each with a semicolon. Here is an example of a Dataproc API snippet that uses a QueryList to specify a HiveJob: "hiveJob": { "queryList": { "queries": [ "query1", "query2", "query3;query4", ] } }</rdfs:comment>
    <rdfs:domain rdf:resource="http://example.org/onto/class/google_dataproc_workflow_template"/>
    <rdfs:range rdf:resource="http://www.w3.org/2001/XMLSchema#string"/>
  </owl:DatatypeProperty>
  <owl:DatatypeProperty rdf:about="http://example.org/onto/prop/google_dataproc_workflow_template_description">
    <rdfs:label>description</rdfs:label>
    <rdfs:comment>Optional. Brief description of the parameter. Must not exceed 1024 characters.</rdfs:comment>
    <rdfs:domain rdf:resource="http://example.org/onto/class/google_dataproc_workflow_template"/>
    <rdfs:range rdf:resource="http://www.w3.org/2001/XMLSchema#string"/>
  </owl:DatatypeProperty>
  <owl:DatatypeProperty rdf:about="http://example.org/onto/prop/google_dataproc_workflow_template_fields">
    <rdfs:label>fields</rdfs:label>
    <rdfs:comment>Required. Paths to all fields that the parameter replaces. A field is allowed to appear in at most one parameter's list of field paths. A field path is similar in syntax to a google.protobuf.FieldMask. For example, a field path that references the zone field of a workflow template's cluster selector would be specified as `placement.clusterSelector.zone`. Also, field paths can reference fields using the following syntax: * Values in maps can be referenced by key: * labels['key'] * placement.clusterSelector.clusterLabels['key'] * placement.managedCluster.labels['key'] * placement.clusterSelector.clusterLabels['key'] * jobs['step-id'].labels['key'] * Jobs in the jobs list can be referenced by step-id: * jobs['step-id'].hadoopJob.mainJarFileUri * jobs['step-id'].hiveJob.queryFileUri * jobs['step-id'].pySparkJob.mainPythonFileUri * jobs['step-id'].hadoopJob.jarFileUris[0] * jobs['step-id'].hadoopJob.archiveUris[0] * jobs['step-id'].hadoopJob.fileUris[0] * jobs['step-id'].pySparkJob.pythonFileUris[0] * Items in repeated fields can be referenced by a zero-based index: * jobs['step-id'].sparkJob.args[0] * Other examples: * jobs['step-id'].hadoopJob.properties['key'] * jobs['step-id'].hadoopJob.args[0] * jobs['step-id'].hiveJob.scriptVariables['key'] * jobs['step-id'].hadoopJob.mainJarFileUri * placement.clusterSelector.zone It may not be possible to parameterize maps and repeated fields in their entirety since only individual map values and individual items in repeated fields can be referenced. For example, the following field paths are invalid: - placement.clusterSelector.clusterLabels - jobs['step-id'].sparkJob.args</rdfs:comment>
    <rdfs:domain rdf:resource="http://example.org/onto/class/google_dataproc_workflow_template"/>
    <rdfs:range rdf:resource="http://www.w3.org/2001/XMLSchema#string"/>
  </owl:DatatypeProperty>
  <owl:DatatypeProperty rdf:about="http://example.org/onto/prop/google_dataproc_workflow_template_name">
    <rdfs:label>name</rdfs:label>
    <rdfs:comment>Required. Parameter name. The parameter name is used as the key, and paired with the parameter value, which are passed to the template when the template is instantiated. The name must contain only capital letters (A-Z), numbers (0-9), and underscores (_), and must not start with a number. The maximum length is 40 characters.</rdfs:comment>
    <rdfs:domain rdf:resource="http://example.org/onto/class/google_dataproc_workflow_template"/>
    <rdfs:range rdf:resource="http://www.w3.org/2001/XMLSchema#string"/>
  </owl:DatatypeProperty>
  <owl:DatatypeProperty rdf:about="http://example.org/onto/prop/google_dataproc_workflow_template_regexes">
    <rdfs:label>regexes</rdfs:label>
    <rdfs:comment>Required. RE2 regular expressions used to validate the parameter's value. The value must match the regex in its entirety (substring matches are not sufficient).</rdfs:comment>
    <rdfs:domain rdf:resource="http://example.org/onto/class/google_dataproc_workflow_template"/>
    <rdfs:range rdf:resource="http://www.w3.org/2001/XMLSchema#string"/>
  </owl:DatatypeProperty>
  <owl:DatatypeProperty rdf:about="http://example.org/onto/prop/google_dataproc_workflow_template_values">
    <rdfs:label>values</rdfs:label>
    <rdfs:comment>Required. List of allowed values for the parameter.</rdfs:comment>
    <rdfs:domain rdf:resource="http://example.org/onto/class/google_dataproc_workflow_template"/>
    <rdfs:range rdf:resource="http://www.w3.org/2001/XMLSchema#string"/>
  </owl:DatatypeProperty>
  <owl:DatatypeProperty rdf:about="http://example.org/onto/prop/google_dataproc_workflow_template_cluster_labels">
    <rdfs:label>cluster_labels</rdfs:label>
    <rdfs:comment>Required. The cluster labels. Cluster must have all labels to match.</rdfs:comment>
    <rdfs:domain rdf:resource="http://example.org/onto/class/google_dataproc_workflow_template"/>
    <rdfs:range rdf:resource="http://www.w3.org/2001/XMLSchema#string"/>
  </owl:DatatypeProperty>
  <owl:DatatypeProperty rdf:about="http://example.org/onto/prop/google_dataproc_workflow_template_zone">
    <rdfs:label>zone</rdfs:label>
    <rdfs:comment>Optional. The zone where workflow process executes. This parameter does not affect the selection of the cluster. If unspecified, the zone of the first cluster matching the selector is used.</rdfs:comment>
    <rdfs:domain rdf:resource="http://example.org/onto/class/google_dataproc_workflow_template"/>
    <rdfs:range rdf:resource="http://www.w3.org/2001/XMLSchema#string"/>
  </owl:DatatypeProperty>
  <owl:DatatypeProperty rdf:about="http://example.org/onto/prop/google_dataproc_workflow_template_cluster_name">
    <rdfs:label>cluster_name</rdfs:label>
    <rdfs:comment>Required. The cluster name prefix. A unique cluster name will be formed by appending a random suffix. The name must contain only lower-case letters (a-z), numbers (0-9), and hyphens (-). Must begin with a letter. Cannot begin or end with hyphen. Must consist of between 2 and 35 characters.</rdfs:comment>
    <rdfs:domain rdf:resource="http://example.org/onto/class/google_dataproc_workflow_template"/>
    <rdfs:range rdf:resource="http://www.w3.org/2001/XMLSchema#string"/>
  </owl:DatatypeProperty>
  <owl:DatatypeProperty rdf:about="http://example.org/onto/prop/google_dataproc_workflow_template_labels">
    <rdfs:label>labels</rdfs:label>
    <rdfs:comment>Optional. The labels to associate with this cluster. Label keys must be between 1 and 63 characters long, and must conform to the following PCRE regular expression: p{Ll}p{Lo}{0,62} Label values must be between 1 and 63 characters long, and must conform to the following PCRE regular expression: [p{Ll}p{Lo}p{N}_-]{0,63} No more than 32 labels can be associated with a given cluster.</rdfs:comment>
    <rdfs:domain rdf:resource="http://example.org/onto/class/google_dataproc_workflow_template"/>
    <rdfs:range rdf:resource="http://www.w3.org/2001/XMLSchema#string"/>
  </owl:DatatypeProperty>
  <owl:DatatypeProperty rdf:about="http://example.org/onto/prop/google_dataproc_workflow_template_staging_bucket">
    <rdfs:label>staging_bucket</rdfs:label>
    <rdfs:comment>Optional. A Cloud Storage bucket used to stage job dependencies, config files, and job driver console output. If you do not specify a staging bucket, Cloud Dataproc will determine a Cloud Storage location (US, ASIA, or EU) for your cluster's staging bucket according to the Compute Engine zone where your cluster is deployed, and then create and manage this project-level, per-location bucket (see [Dataproc staging bucket](https://cloud.google.com/dataproc/docs/concepts/configuring-clusters/staging-bucket)). **This field requires a Cloud Storage bucket name, not a URI to a Cloud Storage bucket.**</rdfs:comment>
    <rdfs:domain rdf:resource="http://example.org/onto/class/google_dataproc_workflow_template"/>
    <rdfs:range rdf:resource="http://www.w3.org/2001/XMLSchema#string"/>
  </owl:DatatypeProperty>
  <owl:DatatypeProperty rdf:about="http://example.org/onto/prop/google_dataproc_workflow_template_temp_bucket">
    <rdfs:label>temp_bucket</rdfs:label>
    <rdfs:comment>Optional. A Cloud Storage bucket used to store ephemeral cluster and jobs data, such as Spark and MapReduce history files. If you do not specify a temp bucket, Dataproc will determine a Cloud Storage location (US, ASIA, or EU) for your cluster's temp bucket according to the Compute Engine zone where your cluster is deployed, and then create and manage this project-level, per-location bucket. The default bucket has a TTL of 90 days, but you can use any TTL (or none) if you specify a bucket. **This field requires a Cloud Storage bucket name, not a URI to a Cloud Storage bucket.**</rdfs:comment>
    <rdfs:domain rdf:resource="http://example.org/onto/class/google_dataproc_workflow_template"/>
    <rdfs:range rdf:resource="http://www.w3.org/2001/XMLSchema#string"/>
  </owl:DatatypeProperty>
  <owl:DatatypeProperty rdf:about="http://example.org/onto/prop/google_dataproc_workflow_template_policy">
    <rdfs:label>policy</rdfs:label>
    <rdfs:comment>Optional. The autoscaling policy used by the cluster. Only resource names including projectid and location (region) are valid. Examples: * `https://www.googleapis.com/compute/v1/projects/[project_id]/locations/[dataproc_region]/autoscalingPolicies/[policy_id]` * `projects/[project_id]/locations/[dataproc_region]/autoscalingPolicies/[policy_id]` Note that the policy must be in the same project and Dataproc region.</rdfs:comment>
    <rdfs:domain rdf:resource="http://example.org/onto/class/google_dataproc_workflow_template"/>
    <rdfs:range rdf:resource="http://www.w3.org/2001/XMLSchema#string"/>
  </owl:DatatypeProperty>
  <owl:DatatypeProperty rdf:about="http://example.org/onto/prop/google_dataproc_workflow_template_gce_pd_kms_key_name">
    <rdfs:label>gce_pd_kms_key_name</rdfs:label>
    <rdfs:comment>Optional. The Cloud KMS key name to use for PD disk encryption for all instances in the cluster.</rdfs:comment>
    <rdfs:domain rdf:resource="http://example.org/onto/class/google_dataproc_workflow_template"/>
    <rdfs:range rdf:resource="http://www.w3.org/2001/XMLSchema#string"/>
  </owl:DatatypeProperty>
  <owl:DatatypeProperty rdf:about="http://example.org/onto/prop/google_dataproc_workflow_template_enable_http_port_access">
    <rdfs:label>enable_http_port_access</rdfs:label>
    <rdfs:comment>Optional. If true, enable http access to specific ports on the cluster from external sources. Defaults to false.</rdfs:comment>
    <rdfs:domain rdf:resource="http://example.org/onto/class/google_dataproc_workflow_template"/>
    <rdfs:range rdf:resource="http://www.w3.org/2001/XMLSchema#string"/>
  </owl:DatatypeProperty>
  <owl:DatatypeProperty rdf:about="http://example.org/onto/prop/google_dataproc_workflow_template_http_ports">
    <rdfs:label>http_ports</rdfs:label>
    <rdfs:comment>Output only. The map of port descriptions to URLs. Will only be populated if enable_http_port_access is true.</rdfs:comment>
    <rdfs:domain rdf:resource="http://example.org/onto/class/google_dataproc_workflow_template"/>
    <rdfs:range rdf:resource="http://www.w3.org/2001/XMLSchema#string"/>
  </owl:DatatypeProperty>
  <owl:DatatypeProperty rdf:about="http://example.org/onto/prop/google_dataproc_workflow_template_internal_ip_only">
    <rdfs:label>internal_ip_only</rdfs:label>
    <rdfs:comment>Optional. If true, all instances in the cluster will only have internal IP addresses. By default, clusters are not restricted to internal IP addresses, and will have ephemeral external IP addresses assigned to each instance. This `internal_ip_only` restriction can only be enabled for subnetwork enabled networks, and all off-cluster dependencies must be configured to be accessible without external IP addresses.</rdfs:comment>
    <rdfs:domain rdf:resource="http://example.org/onto/class/google_dataproc_workflow_template"/>
    <rdfs:range rdf:resource="http://www.w3.org/2001/XMLSchema#string"/>
  </owl:DatatypeProperty>
  <owl:DatatypeProperty rdf:about="http://example.org/onto/prop/google_dataproc_workflow_template_metadata">
    <rdfs:label>metadata</rdfs:label>
    <rdfs:comment>The Compute Engine metadata entries to add to all instances (see [Project and instance metadata](https://cloud.google.com/compute/docs/storing-retrieving-metadata#project_and_instance_metadata)).</rdfs:comment>
    <rdfs:domain rdf:resource="http://example.org/onto/class/google_dataproc_workflow_template"/>
    <rdfs:range rdf:resource="http://www.w3.org/2001/XMLSchema#string"/>
  </owl:DatatypeProperty>
  <owl:DatatypeProperty rdf:about="http://example.org/onto/prop/google_dataproc_workflow_template_network">
    <rdfs:label>network</rdfs:label>
    <rdfs:comment>Optional. The Compute Engine network to be used for machine communications. Cannot be specified with subnetwork_uri. If neither `network_uri` nor `subnetwork_uri` is specified, the "default" network of the project is used, if it exists. Cannot be a "Custom Subnet Network" (see [Using Subnetworks](https://cloud.google.com/compute/docs/subnetworks) for more information). A full URL, partial URI, or short name are valid. Examples: * `https://www.googleapis.com/compute/v1/projects/[project_id]/regions/global/default` * `projects/[project_id]/regions/global/default` * `default`</rdfs:comment>
    <rdfs:domain rdf:resource="http://example.org/onto/class/google_dataproc_workflow_template"/>
    <rdfs:range rdf:resource="http://www.w3.org/2001/XMLSchema#string"/>
  </owl:DatatypeProperty>
  <owl:DatatypeProperty rdf:about="http://example.org/onto/prop/google_dataproc_workflow_template_private_ipv6_google_access">
    <rdfs:label>private_ipv6_google_access</rdfs:label>
    <rdfs:comment>Optional. The type of IPv6 access for a cluster. Possible values: PRIVATE_IPV6_GOOGLE_ACCESS_UNSPECIFIED, INHERIT_FROM_SUBNETWORK, OUTBOUND, BIDIRECTIONAL</rdfs:comment>
    <rdfs:domain rdf:resource="http://example.org/onto/class/google_dataproc_workflow_template"/>
    <rdfs:range rdf:resource="http://www.w3.org/2001/XMLSchema#string"/>
  </owl:DatatypeProperty>
  <owl:DatatypeProperty rdf:about="http://example.org/onto/prop/google_dataproc_workflow_template_service_account">
    <rdfs:label>service_account</rdfs:label>
    <rdfs:comment>Optional. The [Dataproc service account](https://cloud.google.com/dataproc/docs/concepts/configuring-clusters/service-accounts#service_accounts_in_dataproc) (also see [VM Data Plane identity](https://cloud.google.com/dataproc/docs/concepts/iam/dataproc-principals#vm_service_account_data_plane_identity)) used by Dataproc cluster VM instances to access Google Cloud Platform services. If not specified, the [Compute Engine default service account](https://cloud.google.com/compute/docs/access/service-accounts#default_service_account) is used.</rdfs:comment>
    <rdfs:domain rdf:resource="http://example.org/onto/class/google_dataproc_workflow_template"/>
    <rdfs:range rdf:resource="http://www.w3.org/2001/XMLSchema#string"/>
  </owl:DatatypeProperty>
  <owl:DatatypeProperty rdf:about="http://example.org/onto/prop/google_dataproc_workflow_template_service_account_scopes">
    <rdfs:label>service_account_scopes</rdfs:label>
    <rdfs:comment>Optional. The URIs of service account scopes to be included in Compute Engine instances. The following base set of scopes is always included: * https://www.googleapis.com/auth/cloud.useraccounts.readonly * https://www.googleapis.com/auth/devstorage.read_write * https://www.googleapis.com/auth/logging.write If no scopes are specified, the following defaults are also provided: * https://www.googleapis.com/auth/bigquery * https://www.googleapis.com/auth/bigtable.admin.table * https://www.googleapis.com/auth/bigtable.data * https://www.googleapis.com/auth/devstorage.full_control</rdfs:comment>
    <rdfs:domain rdf:resource="http://example.org/onto/class/google_dataproc_workflow_template"/>
    <rdfs:range rdf:resource="http://www.w3.org/2001/XMLSchema#string"/>
  </owl:DatatypeProperty>
  <owl:DatatypeProperty rdf:about="http://example.org/onto/prop/google_dataproc_workflow_template_subnetwork">
    <rdfs:label>subnetwork</rdfs:label>
    <rdfs:comment>Optional. The Compute Engine subnetwork to be used for machine communications. Cannot be specified with network_uri. A full URL, partial URI, or short name are valid. Examples: * `https://www.googleapis.com/compute/v1/projects/[project_id]/regions/us-east1/subnetworks/sub0` * `projects/[project_id]/regions/us-east1/subnetworks/sub0` * `sub0`</rdfs:comment>
    <rdfs:domain rdf:resource="http://example.org/onto/class/google_dataproc_workflow_template"/>
    <rdfs:range rdf:resource="http://www.w3.org/2001/XMLSchema#string"/>
  </owl:DatatypeProperty>
  <owl:DatatypeProperty rdf:about="http://example.org/onto/prop/google_dataproc_workflow_template_tags">
    <rdfs:label>tags</rdfs:label>
    <rdfs:comment>The Compute Engine tags to add to all instances (see [Tagging instances](https://cloud.google.com/compute/docs/label-or-tag-resources#tags)).</rdfs:comment>
    <rdfs:domain rdf:resource="http://example.org/onto/class/google_dataproc_workflow_template"/>
    <rdfs:range rdf:resource="http://www.w3.org/2001/XMLSchema#string"/>
  </owl:DatatypeProperty>
  <owl:DatatypeProperty rdf:about="http://example.org/onto/prop/google_dataproc_workflow_template_zone">
    <rdfs:label>zone</rdfs:label>
    <rdfs:comment>Optional. The zone where the Compute Engine cluster will be located. On a create request, it is required in the "global" region. If omitted in a non-global Dataproc region, the service will pick a zone in the corresponding Compute Engine region. On a get request, zone will always be present. A full URL, partial URI, or short name are valid. Examples: * `https://www.googleapis.com/compute/v1/projects/[project_id]/zones/[zone]` * `projects/[project_id]/zones/[zone]` * `us-central1-f`</rdfs:comment>
    <rdfs:domain rdf:resource="http://example.org/onto/class/google_dataproc_workflow_template"/>
    <rdfs:range rdf:resource="http://www.w3.org/2001/XMLSchema#string"/>
  </owl:DatatypeProperty>
  <owl:DatatypeProperty rdf:about="http://example.org/onto/prop/google_dataproc_workflow_template_node_group">
    <rdfs:label>node_group</rdfs:label>
    <rdfs:comment>Required. The URI of a sole-tenant [node group resource](https://cloud.google.com/compute/docs/reference/rest/v1/nodeGroups) that the cluster will be created on. A full URL, partial URI, or node group name are valid. Examples: * `https://www.googleapis.com/compute/v1/projects/[project_id]/zones/us-central1-a/nodeGroups/node-group-1` * `projects/[project_id]/zones/us-central1-a/nodeGroups/node-group-1` * `node-group-1`</rdfs:comment>
    <rdfs:domain rdf:resource="http://example.org/onto/class/google_dataproc_workflow_template"/>
    <rdfs:range rdf:resource="http://www.w3.org/2001/XMLSchema#string"/>
  </owl:DatatypeProperty>
  <owl:DatatypeProperty rdf:about="http://example.org/onto/prop/google_dataproc_workflow_template_consume_reservation_type">
    <rdfs:label>consume_reservation_type</rdfs:label>
    <rdfs:comment>Optional. Type of reservation to consume Possible values: TYPE_UNSPECIFIED, NO_RESERVATION, ANY_RESERVATION, SPECIFIC_RESERVATION</rdfs:comment>
    <rdfs:domain rdf:resource="http://example.org/onto/class/google_dataproc_workflow_template"/>
    <rdfs:range rdf:resource="http://www.w3.org/2001/XMLSchema#string"/>
  </owl:DatatypeProperty>
  <owl:DatatypeProperty rdf:about="http://example.org/onto/prop/google_dataproc_workflow_template_key">
    <rdfs:label>key</rdfs:label>
    <rdfs:comment>Optional. Corresponds to the label key of reservation resource.</rdfs:comment>
    <rdfs:domain rdf:resource="http://example.org/onto/class/google_dataproc_workflow_template"/>
    <rdfs:range rdf:resource="http://www.w3.org/2001/XMLSchema#string"/>
  </owl:DatatypeProperty>
  <owl:DatatypeProperty rdf:about="http://example.org/onto/prop/google_dataproc_workflow_template_values">
    <rdfs:label>values</rdfs:label>
    <rdfs:comment>Optional. Corresponds to the label values of reservation resource.</rdfs:comment>
    <rdfs:domain rdf:resource="http://example.org/onto/class/google_dataproc_workflow_template"/>
    <rdfs:range rdf:resource="http://www.w3.org/2001/XMLSchema#string"/>
  </owl:DatatypeProperty>
  <owl:DatatypeProperty rdf:about="http://example.org/onto/prop/google_dataproc_workflow_template_enable_integrity_monitoring">
    <rdfs:label>enable_integrity_monitoring</rdfs:label>
    <rdfs:comment>Optional. Defines whether instances have integrity monitoring enabled. Integrity monitoring compares the most recent boot measurements to the integrity policy baseline and returns a pair of pass/fail results depending on whether they match or not.</rdfs:comment>
    <rdfs:domain rdf:resource="http://example.org/onto/class/google_dataproc_workflow_template"/>
    <rdfs:range rdf:resource="http://www.w3.org/2001/XMLSchema#string"/>
  </owl:DatatypeProperty>
  <owl:DatatypeProperty rdf:about="http://example.org/onto/prop/google_dataproc_workflow_template_enable_secure_boot">
    <rdfs:label>enable_secure_boot</rdfs:label>
    <rdfs:comment>Optional. Defines whether the instances have Secure Boot enabled. Secure Boot helps ensure that the system only runs authentic software by verifying the digital signature of all boot components, and halting the boot process if signature verification fails.</rdfs:comment>
    <rdfs:domain rdf:resource="http://example.org/onto/class/google_dataproc_workflow_template"/>
    <rdfs:range rdf:resource="http://www.w3.org/2001/XMLSchema#string"/>
  </owl:DatatypeProperty>
  <owl:DatatypeProperty rdf:about="http://example.org/onto/prop/google_dataproc_workflow_template_enable_vtpm">
    <rdfs:label>enable_vtpm</rdfs:label>
    <rdfs:comment>Optional. Defines whether the instance have the vTPM enabled. Virtual Trusted Platform Module protects objects like keys, certificates and enables Measured Boot by performing the measurements needed to create a known good boot baseline, called the integrity policy baseline.</rdfs:comment>
    <rdfs:domain rdf:resource="http://example.org/onto/class/google_dataproc_workflow_template"/>
    <rdfs:range rdf:resource="http://www.w3.org/2001/XMLSchema#string"/>
  </owl:DatatypeProperty>
  <owl:DatatypeProperty rdf:about="http://example.org/onto/prop/google_dataproc_workflow_template_executable_file">
    <rdfs:label>executable_file</rdfs:label>
    <rdfs:comment>Required. Cloud Storage URI of executable file.</rdfs:comment>
    <rdfs:domain rdf:resource="http://example.org/onto/class/google_dataproc_workflow_template"/>
    <rdfs:range rdf:resource="http://www.w3.org/2001/XMLSchema#string"/>
  </owl:DatatypeProperty>
  <owl:DatatypeProperty rdf:about="http://example.org/onto/prop/google_dataproc_workflow_template_execution_timeout">
    <rdfs:label>execution_timeout</rdfs:label>
    <rdfs:comment>Optional. Amount of time executable has to complete. Default is 10 minutes (see JSON representation of [Duration](https://developers.google.com/protocol-buffers/docs/proto3#json)). Cluster creation fails with an explanatory error message (the name of the executable that caused the error and the exceeded timeout period) if the executable is not completed at end of the timeout period.</rdfs:comment>
    <rdfs:domain rdf:resource="http://example.org/onto/class/google_dataproc_workflow_template"/>
    <rdfs:range rdf:resource="http://www.w3.org/2001/XMLSchema#string"/>
  </owl:DatatypeProperty>
  <owl:DatatypeProperty rdf:about="http://example.org/onto/prop/google_dataproc_workflow_template_auto_delete_time">
    <rdfs:label>auto_delete_time</rdfs:label>
    <rdfs:comment>Optional. The time when cluster will be auto-deleted (see JSON representation of [Timestamp](https://developers.google.com/protocol-buffers/docs/proto3#json)).</rdfs:comment>
    <rdfs:domain rdf:resource="http://example.org/onto/class/google_dataproc_workflow_template"/>
    <rdfs:range rdf:resource="http://www.w3.org/2001/XMLSchema#string"/>
  </owl:DatatypeProperty>
  <owl:DatatypeProperty rdf:about="http://example.org/onto/prop/google_dataproc_workflow_template_auto_delete_ttl">
    <rdfs:label>auto_delete_ttl</rdfs:label>
    <rdfs:comment>Optional. The lifetime duration of cluster. The cluster will be auto-deleted at the end of this period. Minimum value is 10 minutes; maximum value is 14 days (see JSON representation of [Duration](https://developers.google.com/protocol-buffers/docs/proto3#json)).</rdfs:comment>
    <rdfs:domain rdf:resource="http://example.org/onto/class/google_dataproc_workflow_template"/>
    <rdfs:range rdf:resource="http://www.w3.org/2001/XMLSchema#string"/>
  </owl:DatatypeProperty>
  <owl:DatatypeProperty rdf:about="http://example.org/onto/prop/google_dataproc_workflow_template_idle_delete_ttl">
    <rdfs:label>idle_delete_ttl</rdfs:label>
    <rdfs:comment>Optional. The duration to keep the cluster alive while idling (when no jobs are running). Passing this threshold will cause the cluster to be deleted. Minimum value is 5 minutes; maximum value is 14 days (see JSON representation of [Duration](https://developers.google.com/protocol-buffers/docs/proto3#json)).</rdfs:comment>
    <rdfs:domain rdf:resource="http://example.org/onto/class/google_dataproc_workflow_template"/>
    <rdfs:range rdf:resource="http://www.w3.org/2001/XMLSchema#string"/>
  </owl:DatatypeProperty>
  <owl:DatatypeProperty rdf:about="http://example.org/onto/prop/google_dataproc_workflow_template_idle_start_time">
    <rdfs:label>idle_start_time</rdfs:label>
    <rdfs:comment>Output only. The time when cluster became idle (most recent job finished) and became eligible for deletion due to idleness (see JSON representation of [Timestamp](https://developers.google.com/protocol-buffers/docs/proto3#json)).</rdfs:comment>
    <rdfs:domain rdf:resource="http://example.org/onto/class/google_dataproc_workflow_template"/>
    <rdfs:range rdf:resource="http://www.w3.org/2001/XMLSchema#string"/>
  </owl:DatatypeProperty>
  <owl:DatatypeProperty rdf:about="http://example.org/onto/prop/google_dataproc_workflow_template_image">
    <rdfs:label>image</rdfs:label>
    <rdfs:comment>Optional. The Compute Engine image resource used for cluster instances. The URI can represent an image or image family. Image examples: * `https://www.googleapis.com/compute/beta/projects/[project_id]/global/images/[image-id]` * `projects/[project_id]/global/images/[image-id]` * `image-id` Image family examples. Dataproc will use the most recent image from the family: * `https://www.googleapis.com/compute/beta/projects/[project_id]/global/images/family/[custom-image-family-name]` * `projects/[project_id]/global/images/family/[custom-image-family-name]` If the URI is unspecified, it will be inferred from `SoftwareConfig.image_version` or the system default.</rdfs:comment>
    <rdfs:domain rdf:resource="http://example.org/onto/class/google_dataproc_workflow_template"/>
    <rdfs:range rdf:resource="http://www.w3.org/2001/XMLSchema#string"/>
  </owl:DatatypeProperty>
  <owl:DatatypeProperty rdf:about="http://example.org/onto/prop/google_dataproc_workflow_template_instance_names">
    <rdfs:label>instance_names</rdfs:label>
    <rdfs:comment>Output only. The list of instance names. Dataproc derives the names from `cluster_name`, `num_instances`, and the instance group.</rdfs:comment>
    <rdfs:domain rdf:resource="http://example.org/onto/class/google_dataproc_workflow_template"/>
    <rdfs:range rdf:resource="http://www.w3.org/2001/XMLSchema#string"/>
  </owl:DatatypeProperty>
  <owl:DatatypeProperty rdf:about="http://example.org/onto/prop/google_dataproc_workflow_template_is_preemptible">
    <rdfs:label>is_preemptible</rdfs:label>
    <rdfs:comment>Output only. Specifies that this instance group contains preemptible instances.</rdfs:comment>
    <rdfs:domain rdf:resource="http://example.org/onto/class/google_dataproc_workflow_template"/>
    <rdfs:range rdf:resource="http://www.w3.org/2001/XMLSchema#string"/>
  </owl:DatatypeProperty>
  <owl:DatatypeProperty rdf:about="http://example.org/onto/prop/google_dataproc_workflow_template_machine_type">
    <rdfs:label>machine_type</rdfs:label>
    <rdfs:comment>Optional. The Compute Engine machine type used for cluster instances. A full URL, partial URI, or short name are valid. Examples: * `https://www.googleapis.com/compute/v1/projects/[project_id]/zones/us-east1-a/machineTypes/n1-standard-2` * `projects/[project_id]/zones/us-east1-a/machineTypes/n1-standard-2` * `n1-standard-2` **Auto Zone Exception**: If you are using the Dataproc [Auto Zone Placement](https://cloud.google.com/dataproc/docs/concepts/configuring-clusters/auto-zone#using_auto_zone_placement) feature, you must use the short name of the machine type resource, for example, `n1-standard-2`.</rdfs:comment>
    <rdfs:domain rdf:resource="http://example.org/onto/class/google_dataproc_workflow_template"/>
    <rdfs:range rdf:resource="http://www.w3.org/2001/XMLSchema#string"/>
  </owl:DatatypeProperty>
  <owl:DatatypeProperty rdf:about="http://example.org/onto/prop/google_dataproc_workflow_template_managed_group_config">
    <rdfs:label>managed_group_config</rdfs:label>
    <rdfs:comment>Output only. The config for Compute Engine Instance Group Manager that manages this group. This is only used for preemptible instance groups.</rdfs:comment>
    <rdfs:domain rdf:resource="http://example.org/onto/class/google_dataproc_workflow_template"/>
    <rdfs:range rdf:resource="http://www.w3.org/2001/XMLSchema#string"/>
  </owl:DatatypeProperty>
  <owl:DatatypeProperty rdf:about="http://example.org/onto/prop/google_dataproc_workflow_template_min_cpu_platform">
    <rdfs:label>min_cpu_platform</rdfs:label>
    <rdfs:comment>Optional. Specifies the minimum cpu platform for the Instance Group. See [Dataproc -> Minimum CPU Platform](https://cloud.google.com/dataproc/docs/concepts/compute/dataproc-min-cpu).</rdfs:comment>
    <rdfs:domain rdf:resource="http://example.org/onto/class/google_dataproc_workflow_template"/>
    <rdfs:range rdf:resource="http://www.w3.org/2001/XMLSchema#string"/>
  </owl:DatatypeProperty>
  <owl:DatatypeProperty rdf:about="http://example.org/onto/prop/google_dataproc_workflow_template_num_instances">
    <rdfs:label>num_instances</rdfs:label>
    <rdfs:comment>Optional. The number of VM instances in the instance group. For [HA cluster](/dataproc/docs/concepts/configuring-clusters/high-availability) [master_config](#FIELDS.master_config) groups, **must be set to 3**. For standard cluster [master_config](#FIELDS.master_config) groups, **must be set to 1**.</rdfs:comment>
    <rdfs:domain rdf:resource="http://example.org/onto/class/google_dataproc_workflow_template"/>
    <rdfs:range rdf:resource="http://www.w3.org/2001/XMLSchema#string"/>
  </owl:DatatypeProperty>
  <owl:DatatypeProperty rdf:about="http://example.org/onto/prop/google_dataproc_workflow_template_preemptibility">
    <rdfs:label>preemptibility</rdfs:label>
    <rdfs:comment>Optional. Specifies the preemptibility of the instance group. The default value for master and worker groups is `NON_PREEMPTIBLE`. This default cannot be changed. The default value for secondary instances is `PREEMPTIBLE`. Possible values: PREEMPTIBILITY_UNSPECIFIED, NON_PREEMPTIBLE, PREEMPTIBLE</rdfs:comment>
    <rdfs:domain rdf:resource="http://example.org/onto/class/google_dataproc_workflow_template"/>
    <rdfs:range rdf:resource="http://www.w3.org/2001/XMLSchema#string"/>
  </owl:DatatypeProperty>
  <owl:DatatypeProperty rdf:about="http://example.org/onto/prop/google_dataproc_workflow_template_accelerator_count">
    <rdfs:label>accelerator_count</rdfs:label>
    <rdfs:comment>The number of the accelerator cards of this type exposed to this instance.</rdfs:comment>
    <rdfs:domain rdf:resource="http://example.org/onto/class/google_dataproc_workflow_template"/>
    <rdfs:range rdf:resource="http://www.w3.org/2001/XMLSchema#string"/>
  </owl:DatatypeProperty>
  <owl:DatatypeProperty rdf:about="http://example.org/onto/prop/google_dataproc_workflow_template_accelerator_type">
    <rdfs:label>accelerator_type</rdfs:label>
    <rdfs:comment>Full URL, partial URI, or short name of the accelerator type resource to expose to this instance. See [Compute Engine AcceleratorTypes](https://cloud.google.com/compute/docs/reference/beta/acceleratorTypes). Examples: * `https://www.googleapis.com/compute/beta/projects/[project_id]/zones/us-east1-a/acceleratorTypes/nvidia-tesla-k80` * `projects/[project_id]/zones/us-east1-a/acceleratorTypes/nvidia-tesla-k80` * `nvidia-tesla-k80` **Auto Zone Exception**: If you are using the Dataproc [Auto Zone Placement](https://cloud.google.com/dataproc/docs/concepts/configuring-clusters/auto-zone#using_auto_zone_placement) feature, you must use the short name of the accelerator type resource, for example, `nvidia-tesla-k80`.</rdfs:comment>
    <rdfs:domain rdf:resource="http://example.org/onto/class/google_dataproc_workflow_template"/>
    <rdfs:range rdf:resource="http://www.w3.org/2001/XMLSchema#string"/>
  </owl:DatatypeProperty>
  <owl:DatatypeProperty rdf:about="http://example.org/onto/prop/google_dataproc_workflow_template_boot_disk_size_gb">
    <rdfs:label>boot_disk_size_gb</rdfs:label>
    <rdfs:comment>Optional. Size in GB of the boot disk (default is 500GB).</rdfs:comment>
    <rdfs:domain rdf:resource="http://example.org/onto/class/google_dataproc_workflow_template"/>
    <rdfs:range rdf:resource="http://www.w3.org/2001/XMLSchema#string"/>
  </owl:DatatypeProperty>
  <owl:DatatypeProperty rdf:about="http://example.org/onto/prop/google_dataproc_workflow_template_boot_disk_type">
    <rdfs:label>boot_disk_type</rdfs:label>
    <rdfs:comment>Optional. Type of the boot disk (default is "pd-standard"). Valid values: "pd-balanced" (Persistent Disk Balanced Solid State Drive), "pd-ssd" (Persistent Disk Solid State Drive), or "pd-standard" (Persistent Disk Hard Disk Drive). See [Disk types](https://cloud.google.com/compute/docs/disks#disk-types).</rdfs:comment>
    <rdfs:domain rdf:resource="http://example.org/onto/class/google_dataproc_workflow_template"/>
    <rdfs:range rdf:resource="http://www.w3.org/2001/XMLSchema#string"/>
  </owl:DatatypeProperty>
  <owl:DatatypeProperty rdf:about="http://example.org/onto/prop/google_dataproc_workflow_template_num_local_ssds">
    <rdfs:label>num_local_ssds</rdfs:label>
    <rdfs:comment>Optional. Number of attached SSDs, from 0 to 4 (default is 0). If SSDs are not attached, the boot disk is used to store runtime logs and [HDFS](https://hadoop.apache.org/docs/r1.2.1/hdfs_user_guide.html) data. If one or more SSDs are attached, this runtime bulk data is spread across them, and the boot disk contains only basic config and installed binaries.</rdfs:comment>
    <rdfs:domain rdf:resource="http://example.org/onto/class/google_dataproc_workflow_template"/>
    <rdfs:range rdf:resource="http://www.w3.org/2001/XMLSchema#string"/>
  </owl:DatatypeProperty>
  <owl:DatatypeProperty rdf:about="http://example.org/onto/prop/google_dataproc_workflow_template_image">
    <rdfs:label>image</rdfs:label>
    <rdfs:comment>Optional. The Compute Engine image resource used for cluster instances. The URI can represent an image or image family. Image examples: * `https://www.googleapis.com/compute/beta/projects/[project_id]/global/images/[image-id]` * `projects/[project_id]/global/images/[image-id]` * `image-id` Image family examples. Dataproc will use the most recent image from the family: * `https://www.googleapis.com/compute/beta/projects/[project_id]/global/images/family/[custom-image-family-name]` * `projects/[project_id]/global/images/family/[custom-image-family-name]` If the URI is unspecified, it will be inferred from `SoftwareConfig.image_version` or the system default.</rdfs:comment>
    <rdfs:domain rdf:resource="http://example.org/onto/class/google_dataproc_workflow_template"/>
    <rdfs:range rdf:resource="http://www.w3.org/2001/XMLSchema#string"/>
  </owl:DatatypeProperty>
  <owl:DatatypeProperty rdf:about="http://example.org/onto/prop/google_dataproc_workflow_template_instance_names">
    <rdfs:label>instance_names</rdfs:label>
    <rdfs:comment>Output only. The list of instance names. Dataproc derives the names from `cluster_name`, `num_instances`, and the instance group.</rdfs:comment>
    <rdfs:domain rdf:resource="http://example.org/onto/class/google_dataproc_workflow_template"/>
    <rdfs:range rdf:resource="http://www.w3.org/2001/XMLSchema#string"/>
  </owl:DatatypeProperty>
  <owl:DatatypeProperty rdf:about="http://example.org/onto/prop/google_dataproc_workflow_template_is_preemptible">
    <rdfs:label>is_preemptible</rdfs:label>
    <rdfs:comment>Output only. Specifies that this instance group contains preemptible instances.</rdfs:comment>
    <rdfs:domain rdf:resource="http://example.org/onto/class/google_dataproc_workflow_template"/>
    <rdfs:range rdf:resource="http://www.w3.org/2001/XMLSchema#string"/>
  </owl:DatatypeProperty>
  <owl:DatatypeProperty rdf:about="http://example.org/onto/prop/google_dataproc_workflow_template_machine_type">
    <rdfs:label>machine_type</rdfs:label>
    <rdfs:comment>Optional. The Compute Engine machine type used for cluster instances. A full URL, partial URI, or short name are valid. Examples: * `https://www.googleapis.com/compute/v1/projects/[project_id]/zones/us-east1-a/machineTypes/n1-standard-2` * `projects/[project_id]/zones/us-east1-a/machineTypes/n1-standard-2` * `n1-standard-2` **Auto Zone Exception**: If you are using the Dataproc [Auto Zone Placement](https://cloud.google.com/dataproc/docs/concepts/configuring-clusters/auto-zone#using_auto_zone_placement) feature, you must use the short name of the machine type resource, for example, `n1-standard-2`.</rdfs:comment>
    <rdfs:domain rdf:resource="http://example.org/onto/class/google_dataproc_workflow_template"/>
    <rdfs:range rdf:resource="http://www.w3.org/2001/XMLSchema#string"/>
  </owl:DatatypeProperty>
  <owl:DatatypeProperty rdf:about="http://example.org/onto/prop/google_dataproc_workflow_template_managed_group_config">
    <rdfs:label>managed_group_config</rdfs:label>
    <rdfs:comment>Output only. The config for Compute Engine Instance Group Manager that manages this group. This is only used for preemptible instance groups.</rdfs:comment>
    <rdfs:domain rdf:resource="http://example.org/onto/class/google_dataproc_workflow_template"/>
    <rdfs:range rdf:resource="http://www.w3.org/2001/XMLSchema#string"/>
  </owl:DatatypeProperty>
  <owl:DatatypeProperty rdf:about="http://example.org/onto/prop/google_dataproc_workflow_template_min_cpu_platform">
    <rdfs:label>min_cpu_platform</rdfs:label>
    <rdfs:comment>Optional. Specifies the minimum cpu platform for the Instance Group. See [Dataproc -> Minimum CPU Platform](https://cloud.google.com/dataproc/docs/concepts/compute/dataproc-min-cpu).</rdfs:comment>
    <rdfs:domain rdf:resource="http://example.org/onto/class/google_dataproc_workflow_template"/>
    <rdfs:range rdf:resource="http://www.w3.org/2001/XMLSchema#string"/>
  </owl:DatatypeProperty>
  <owl:DatatypeProperty rdf:about="http://example.org/onto/prop/google_dataproc_workflow_template_num_instances">
    <rdfs:label>num_instances</rdfs:label>
    <rdfs:comment>Optional. The number of VM instances in the instance group. For [HA cluster](/dataproc/docs/concepts/configuring-clusters/high-availability) [master_config](#FIELDS.master_config) groups, **must be set to 3**. For standard cluster [master_config](#FIELDS.master_config) groups, **must be set to 1**.</rdfs:comment>
    <rdfs:domain rdf:resource="http://example.org/onto/class/google_dataproc_workflow_template"/>
    <rdfs:range rdf:resource="http://www.w3.org/2001/XMLSchema#string"/>
  </owl:DatatypeProperty>
  <owl:DatatypeProperty rdf:about="http://example.org/onto/prop/google_dataproc_workflow_template_preemptibility">
    <rdfs:label>preemptibility</rdfs:label>
    <rdfs:comment>Optional. Specifies the preemptibility of the instance group. The default value for master and worker groups is `NON_PREEMPTIBLE`. This default cannot be changed. The default value for secondary instances is `PREEMPTIBLE`. Possible values: PREEMPTIBILITY_UNSPECIFIED, NON_PREEMPTIBLE, PREEMPTIBLE</rdfs:comment>
    <rdfs:domain rdf:resource="http://example.org/onto/class/google_dataproc_workflow_template"/>
    <rdfs:range rdf:resource="http://www.w3.org/2001/XMLSchema#string"/>
  </owl:DatatypeProperty>
  <owl:DatatypeProperty rdf:about="http://example.org/onto/prop/google_dataproc_workflow_template_accelerator_count">
    <rdfs:label>accelerator_count</rdfs:label>
    <rdfs:comment>The number of the accelerator cards of this type exposed to this instance.</rdfs:comment>
    <rdfs:domain rdf:resource="http://example.org/onto/class/google_dataproc_workflow_template"/>
    <rdfs:range rdf:resource="http://www.w3.org/2001/XMLSchema#string"/>
  </owl:DatatypeProperty>
  <owl:DatatypeProperty rdf:about="http://example.org/onto/prop/google_dataproc_workflow_template_accelerator_type">
    <rdfs:label>accelerator_type</rdfs:label>
    <rdfs:comment>Full URL, partial URI, or short name of the accelerator type resource to expose to this instance. See [Compute Engine AcceleratorTypes](https://cloud.google.com/compute/docs/reference/beta/acceleratorTypes). Examples: * `https://www.googleapis.com/compute/beta/projects/[project_id]/zones/us-east1-a/acceleratorTypes/nvidia-tesla-k80` * `projects/[project_id]/zones/us-east1-a/acceleratorTypes/nvidia-tesla-k80` * `nvidia-tesla-k80` **Auto Zone Exception**: If you are using the Dataproc [Auto Zone Placement](https://cloud.google.com/dataproc/docs/concepts/configuring-clusters/auto-zone#using_auto_zone_placement) feature, you must use the short name of the accelerator type resource, for example, `nvidia-tesla-k80`.</rdfs:comment>
    <rdfs:domain rdf:resource="http://example.org/onto/class/google_dataproc_workflow_template"/>
    <rdfs:range rdf:resource="http://www.w3.org/2001/XMLSchema#string"/>
  </owl:DatatypeProperty>
  <owl:DatatypeProperty rdf:about="http://example.org/onto/prop/google_dataproc_workflow_template_boot_disk_size_gb">
    <rdfs:label>boot_disk_size_gb</rdfs:label>
    <rdfs:comment>Optional. Size in GB of the boot disk (default is 500GB).</rdfs:comment>
    <rdfs:domain rdf:resource="http://example.org/onto/class/google_dataproc_workflow_template"/>
    <rdfs:range rdf:resource="http://www.w3.org/2001/XMLSchema#string"/>
  </owl:DatatypeProperty>
  <owl:DatatypeProperty rdf:about="http://example.org/onto/prop/google_dataproc_workflow_template_boot_disk_type">
    <rdfs:label>boot_disk_type</rdfs:label>
    <rdfs:comment>Optional. Type of the boot disk (default is "pd-standard"). Valid values: "pd-balanced" (Persistent Disk Balanced Solid State Drive), "pd-ssd" (Persistent Disk Solid State Drive), or "pd-standard" (Persistent Disk Hard Disk Drive). See [Disk types](https://cloud.google.com/compute/docs/disks#disk-types).</rdfs:comment>
    <rdfs:domain rdf:resource="http://example.org/onto/class/google_dataproc_workflow_template"/>
    <rdfs:range rdf:resource="http://www.w3.org/2001/XMLSchema#string"/>
  </owl:DatatypeProperty>
  <owl:DatatypeProperty rdf:about="http://example.org/onto/prop/google_dataproc_workflow_template_num_local_ssds">
    <rdfs:label>num_local_ssds</rdfs:label>
    <rdfs:comment>Optional. Number of attached SSDs, from 0 to 4 (default is 0). If SSDs are not attached, the boot disk is used to store runtime logs and [HDFS](https://hadoop.apache.org/docs/r1.2.1/hdfs_user_guide.html) data. If one or more SSDs are attached, this runtime bulk data is spread across them, and the boot disk contains only basic config and installed binaries.</rdfs:comment>
    <rdfs:domain rdf:resource="http://example.org/onto/class/google_dataproc_workflow_template"/>
    <rdfs:range rdf:resource="http://www.w3.org/2001/XMLSchema#string"/>
  </owl:DatatypeProperty>
  <owl:DatatypeProperty rdf:about="http://example.org/onto/prop/google_dataproc_workflow_template_cross_realm_trust_admin_server">
    <rdfs:label>cross_realm_trust_admin_server</rdfs:label>
    <rdfs:comment>Optional. The admin server (IP or hostname) for the remote trusted realm in a cross realm trust relationship.</rdfs:comment>
    <rdfs:domain rdf:resource="http://example.org/onto/class/google_dataproc_workflow_template"/>
    <rdfs:range rdf:resource="http://www.w3.org/2001/XMLSchema#string"/>
  </owl:DatatypeProperty>
  <owl:DatatypeProperty rdf:about="http://example.org/onto/prop/google_dataproc_workflow_template_cross_realm_trust_kdc">
    <rdfs:label>cross_realm_trust_kdc</rdfs:label>
    <rdfs:comment>Optional. The KDC (IP or hostname) for the remote trusted realm in a cross realm trust relationship.</rdfs:comment>
    <rdfs:domain rdf:resource="http://example.org/onto/class/google_dataproc_workflow_template"/>
    <rdfs:range rdf:resource="http://www.w3.org/2001/XMLSchema#string"/>
  </owl:DatatypeProperty>
  <owl:DatatypeProperty rdf:about="http://example.org/onto/prop/google_dataproc_workflow_template_cross_realm_trust_realm">
    <rdfs:label>cross_realm_trust_realm</rdfs:label>
    <rdfs:comment>Optional. The remote realm the Dataproc on-cluster KDC will trust, should the user enable cross realm trust.</rdfs:comment>
    <rdfs:domain rdf:resource="http://example.org/onto/class/google_dataproc_workflow_template"/>
    <rdfs:range rdf:resource="http://www.w3.org/2001/XMLSchema#string"/>
  </owl:DatatypeProperty>
  <owl:DatatypeProperty rdf:about="http://example.org/onto/prop/google_dataproc_workflow_template_cross_realm_trust_shared_password">
    <rdfs:label>cross_realm_trust_shared_password</rdfs:label>
    <rdfs:comment>Optional. The Cloud Storage URI of a KMS encrypted file containing the shared password between the on-cluster Kerberos realm and the remote trusted realm, in a cross realm trust relationship.</rdfs:comment>
    <rdfs:domain rdf:resource="http://example.org/onto/class/google_dataproc_workflow_template"/>
    <rdfs:range rdf:resource="http://www.w3.org/2001/XMLSchema#string"/>
  </owl:DatatypeProperty>
  <owl:DatatypeProperty rdf:about="http://example.org/onto/prop/google_dataproc_workflow_template_enable_kerberos">
    <rdfs:label>enable_kerberos</rdfs:label>
    <rdfs:comment>Optional. Flag to indicate whether to Kerberize the cluster (default: false). Set this field to true to enable Kerberos on a cluster.</rdfs:comment>
    <rdfs:domain rdf:resource="http://example.org/onto/class/google_dataproc_workflow_template"/>
    <rdfs:range rdf:resource="http://www.w3.org/2001/XMLSchema#string"/>
  </owl:DatatypeProperty>
  <owl:DatatypeProperty rdf:about="http://example.org/onto/prop/google_dataproc_workflow_template_kdc_db_key">
    <rdfs:label>kdc_db_key</rdfs:label>
    <rdfs:comment>Optional. The Cloud Storage URI of a KMS encrypted file containing the master key of the KDC database.</rdfs:comment>
    <rdfs:domain rdf:resource="http://example.org/onto/class/google_dataproc_workflow_template"/>
    <rdfs:range rdf:resource="http://www.w3.org/2001/XMLSchema#string"/>
  </owl:DatatypeProperty>
  <owl:DatatypeProperty rdf:about="http://example.org/onto/prop/google_dataproc_workflow_template_key_password">
    <rdfs:label>key_password</rdfs:label>
    <rdfs:comment>Optional. The Cloud Storage URI of a KMS encrypted file containing the password to the user provided key. For the self-signed certificate, this password is generated by Dataproc.</rdfs:comment>
    <rdfs:domain rdf:resource="http://example.org/onto/class/google_dataproc_workflow_template"/>
    <rdfs:range rdf:resource="http://www.w3.org/2001/XMLSchema#string"/>
  </owl:DatatypeProperty>
  <owl:DatatypeProperty rdf:about="http://example.org/onto/prop/google_dataproc_workflow_template_keystore">
    <rdfs:label>keystore</rdfs:label>
    <rdfs:comment>Optional. The Cloud Storage URI of the keystore file used for SSL encryption. If not provided, Dataproc will provide a self-signed certificate.</rdfs:comment>
    <rdfs:domain rdf:resource="http://example.org/onto/class/google_dataproc_workflow_template"/>
    <rdfs:range rdf:resource="http://www.w3.org/2001/XMLSchema#string"/>
  </owl:DatatypeProperty>
  <owl:DatatypeProperty rdf:about="http://example.org/onto/prop/google_dataproc_workflow_template_keystore_password">
    <rdfs:label>keystore_password</rdfs:label>
    <rdfs:comment>Optional. The Cloud Storage URI of a KMS encrypted file containing the password to the user provided keystore. For the self-signed certificate, this password is generated by Dataproc.</rdfs:comment>
    <rdfs:domain rdf:resource="http://example.org/onto/class/google_dataproc_workflow_template"/>
    <rdfs:range rdf:resource="http://www.w3.org/2001/XMLSchema#string"/>
  </owl:DatatypeProperty>
  <owl:DatatypeProperty rdf:about="http://example.org/onto/prop/google_dataproc_workflow_template_kms_key">
    <rdfs:label>kms_key</rdfs:label>
    <rdfs:comment>Optional. The uri of the KMS key used to encrypt various sensitive files.</rdfs:comment>
    <rdfs:domain rdf:resource="http://example.org/onto/class/google_dataproc_workflow_template"/>
    <rdfs:range rdf:resource="http://www.w3.org/2001/XMLSchema#string"/>
  </owl:DatatypeProperty>
  <owl:DatatypeProperty rdf:about="http://example.org/onto/prop/google_dataproc_workflow_template_realm">
    <rdfs:label>realm</rdfs:label>
    <rdfs:comment>Optional. The name of the on-cluster Kerberos realm. If not specified, the uppercased domain of hostnames will be the realm.</rdfs:comment>
    <rdfs:domain rdf:resource="http://example.org/onto/class/google_dataproc_workflow_template"/>
    <rdfs:range rdf:resource="http://www.w3.org/2001/XMLSchema#string"/>
  </owl:DatatypeProperty>
  <owl:DatatypeProperty rdf:about="http://example.org/onto/prop/google_dataproc_workflow_template_root_principal_password">
    <rdfs:label>root_principal_password</rdfs:label>
    <rdfs:comment>Optional. The Cloud Storage URI of a KMS encrypted file containing the root principal password.</rdfs:comment>
    <rdfs:domain rdf:resource="http://example.org/onto/class/google_dataproc_workflow_template"/>
    <rdfs:range rdf:resource="http://www.w3.org/2001/XMLSchema#string"/>
  </owl:DatatypeProperty>
  <owl:DatatypeProperty rdf:about="http://example.org/onto/prop/google_dataproc_workflow_template_tgt_lifetime_hours">
    <rdfs:label>tgt_lifetime_hours</rdfs:label>
    <rdfs:comment>Optional. The lifetime of the ticket granting ticket, in hours. If not specified, or user specifies 0, then default value 10 will be used.</rdfs:comment>
    <rdfs:domain rdf:resource="http://example.org/onto/class/google_dataproc_workflow_template"/>
    <rdfs:range rdf:resource="http://www.w3.org/2001/XMLSchema#string"/>
  </owl:DatatypeProperty>
  <owl:DatatypeProperty rdf:about="http://example.org/onto/prop/google_dataproc_workflow_template_truststore">
    <rdfs:label>truststore</rdfs:label>
    <rdfs:comment>Optional. The Cloud Storage URI of the truststore file used for SSL encryption. If not provided, Dataproc will provide a self-signed certificate.</rdfs:comment>
    <rdfs:domain rdf:resource="http://example.org/onto/class/google_dataproc_workflow_template"/>
    <rdfs:range rdf:resource="http://www.w3.org/2001/XMLSchema#string"/>
  </owl:DatatypeProperty>
  <owl:DatatypeProperty rdf:about="http://example.org/onto/prop/google_dataproc_workflow_template_truststore_password">
    <rdfs:label>truststore_password</rdfs:label>
    <rdfs:comment>Optional. The Cloud Storage URI of a KMS encrypted file containing the password to the user provided truststore. For the self-signed certificate, this password is generated by Dataproc.</rdfs:comment>
    <rdfs:domain rdf:resource="http://example.org/onto/class/google_dataproc_workflow_template"/>
    <rdfs:range rdf:resource="http://www.w3.org/2001/XMLSchema#string"/>
  </owl:DatatypeProperty>
  <owl:DatatypeProperty rdf:about="http://example.org/onto/prop/google_dataproc_workflow_template_image_version">
    <rdfs:label>image_version</rdfs:label>
    <rdfs:comment>Optional. The version of software inside the cluster. It must be one of the supported [Dataproc Versions](https://cloud.google.com/dataproc/docs/concepts/versioning/dataproc-versions#supported_dataproc_versions), such as "1.2" (including a subminor version, such as "1.2.29"), or the ["preview" version](https://cloud.google.com/dataproc/docs/concepts/versioning/dataproc-versions#other_versions). If unspecified, it defaults to the latest Debian version.</rdfs:comment>
    <rdfs:domain rdf:resource="http://example.org/onto/class/google_dataproc_workflow_template"/>
    <rdfs:range rdf:resource="http://www.w3.org/2001/XMLSchema#string"/>
  </owl:DatatypeProperty>
  <owl:DatatypeProperty rdf:about="http://example.org/onto/prop/google_dataproc_workflow_template_optional_components">
    <rdfs:label>optional_components</rdfs:label>
    <rdfs:comment>Optional. The set of components to activate on the cluster.</rdfs:comment>
    <rdfs:domain rdf:resource="http://example.org/onto/class/google_dataproc_workflow_template"/>
    <rdfs:range rdf:resource="http://www.w3.org/2001/XMLSchema#string"/>
  </owl:DatatypeProperty>
  <owl:DatatypeProperty rdf:about="http://example.org/onto/prop/google_dataproc_workflow_template_properties">
    <rdfs:label>properties</rdfs:label>
    <rdfs:comment>Optional. The properties to set on daemon config files. Property keys are specified in `prefix:property` format, for example `core:hadoop.tmp.dir`. The following are supported prefixes and their mappings: * capacity-scheduler: `capacity-scheduler.xml` * core: `core-site.xml` * distcp: `distcp-default.xml` * hdfs: `hdfs-site.xml` * hive: `hive-site.xml` * mapred: `mapred-site.xml` * pig: `pig.properties` * spark: `spark-defaults.conf` * yarn: `yarn-site.xml` For more information, see [Cluster properties](https://cloud.google.com/dataproc/docs/concepts/cluster-properties).</rdfs:comment>
    <rdfs:domain rdf:resource="http://example.org/onto/class/google_dataproc_workflow_template"/>
    <rdfs:range rdf:resource="http://www.w3.org/2001/XMLSchema#string"/>
  </owl:DatatypeProperty>
  <owl:DatatypeProperty rdf:about="http://example.org/onto/prop/google_dataproc_workflow_template_image">
    <rdfs:label>image</rdfs:label>
    <rdfs:comment>Optional. The Compute Engine image resource used for cluster instances. The URI can represent an image or image family. Image examples: * `https://www.googleapis.com/compute/beta/projects/[project_id]/global/images/[image-id]` * `projects/[project_id]/global/images/[image-id]` * `image-id` Image family examples. Dataproc will use the most recent image from the family: * `https://www.googleapis.com/compute/beta/projects/[project_id]/global/images/family/[custom-image-family-name]` * `projects/[project_id]/global/images/family/[custom-image-family-name]` If the URI is unspecified, it will be inferred from `SoftwareConfig.image_version` or the system default.</rdfs:comment>
    <rdfs:domain rdf:resource="http://example.org/onto/class/google_dataproc_workflow_template"/>
    <rdfs:range rdf:resource="http://www.w3.org/2001/XMLSchema#string"/>
  </owl:DatatypeProperty>
  <owl:DatatypeProperty rdf:about="http://example.org/onto/prop/google_dataproc_workflow_template_instance_names">
    <rdfs:label>instance_names</rdfs:label>
    <rdfs:comment>Output only. The list of instance names. Dataproc derives the names from `cluster_name`, `num_instances`, and the instance group.</rdfs:comment>
    <rdfs:domain rdf:resource="http://example.org/onto/class/google_dataproc_workflow_template"/>
    <rdfs:range rdf:resource="http://www.w3.org/2001/XMLSchema#string"/>
  </owl:DatatypeProperty>
  <owl:DatatypeProperty rdf:about="http://example.org/onto/prop/google_dataproc_workflow_template_is_preemptible">
    <rdfs:label>is_preemptible</rdfs:label>
    <rdfs:comment>Output only. Specifies that this instance group contains preemptible instances.</rdfs:comment>
    <rdfs:domain rdf:resource="http://example.org/onto/class/google_dataproc_workflow_template"/>
    <rdfs:range rdf:resource="http://www.w3.org/2001/XMLSchema#string"/>
  </owl:DatatypeProperty>
  <owl:DatatypeProperty rdf:about="http://example.org/onto/prop/google_dataproc_workflow_template_machine_type">
    <rdfs:label>machine_type</rdfs:label>
    <rdfs:comment>Optional. The Compute Engine machine type used for cluster instances. A full URL, partial URI, or short name are valid. Examples: * `https://www.googleapis.com/compute/v1/projects/[project_id]/zones/us-east1-a/machineTypes/n1-standard-2` * `projects/[project_id]/zones/us-east1-a/machineTypes/n1-standard-2` * `n1-standard-2` **Auto Zone Exception**: If you are using the Dataproc [Auto Zone Placement](https://cloud.google.com/dataproc/docs/concepts/configuring-clusters/auto-zone#using_auto_zone_placement) feature, you must use the short name of the machine type resource, for example, `n1-standard-2`.</rdfs:comment>
    <rdfs:domain rdf:resource="http://example.org/onto/class/google_dataproc_workflow_template"/>
    <rdfs:range rdf:resource="http://www.w3.org/2001/XMLSchema#string"/>
  </owl:DatatypeProperty>
  <owl:DatatypeProperty rdf:about="http://example.org/onto/prop/google_dataproc_workflow_template_managed_group_config">
    <rdfs:label>managed_group_config</rdfs:label>
    <rdfs:comment>Output only. The config for Compute Engine Instance Group Manager that manages this group. This is only used for preemptible instance groups.</rdfs:comment>
    <rdfs:domain rdf:resource="http://example.org/onto/class/google_dataproc_workflow_template"/>
    <rdfs:range rdf:resource="http://www.w3.org/2001/XMLSchema#string"/>
  </owl:DatatypeProperty>
  <owl:DatatypeProperty rdf:about="http://example.org/onto/prop/google_dataproc_workflow_template_min_cpu_platform">
    <rdfs:label>min_cpu_platform</rdfs:label>
    <rdfs:comment>Optional. Specifies the minimum cpu platform for the Instance Group. See [Dataproc -> Minimum CPU Platform](https://cloud.google.com/dataproc/docs/concepts/compute/dataproc-min-cpu).</rdfs:comment>
    <rdfs:domain rdf:resource="http://example.org/onto/class/google_dataproc_workflow_template"/>
    <rdfs:range rdf:resource="http://www.w3.org/2001/XMLSchema#string"/>
  </owl:DatatypeProperty>
  <owl:DatatypeProperty rdf:about="http://example.org/onto/prop/google_dataproc_workflow_template_num_instances">
    <rdfs:label>num_instances</rdfs:label>
    <rdfs:comment>Optional. The number of VM instances in the instance group. For [HA cluster](/dataproc/docs/concepts/configuring-clusters/high-availability) [master_config](#FIELDS.master_config) groups, **must be set to 3**. For standard cluster [master_config](#FIELDS.master_config) groups, **must be set to 1**.</rdfs:comment>
    <rdfs:domain rdf:resource="http://example.org/onto/class/google_dataproc_workflow_template"/>
    <rdfs:range rdf:resource="http://www.w3.org/2001/XMLSchema#string"/>
  </owl:DatatypeProperty>
  <owl:DatatypeProperty rdf:about="http://example.org/onto/prop/google_dataproc_workflow_template_preemptibility">
    <rdfs:label>preemptibility</rdfs:label>
    <rdfs:comment>Optional. Specifies the preemptibility of the instance group. The default value for master and worker groups is `NON_PREEMPTIBLE`. This default cannot be changed. The default value for secondary instances is `PREEMPTIBLE`. Possible values: PREEMPTIBILITY_UNSPECIFIED, NON_PREEMPTIBLE, PREEMPTIBLE</rdfs:comment>
    <rdfs:domain rdf:resource="http://example.org/onto/class/google_dataproc_workflow_template"/>
    <rdfs:range rdf:resource="http://www.w3.org/2001/XMLSchema#string"/>
  </owl:DatatypeProperty>
  <owl:DatatypeProperty rdf:about="http://example.org/onto/prop/google_dataproc_workflow_template_accelerator_count">
    <rdfs:label>accelerator_count</rdfs:label>
    <rdfs:comment>The number of the accelerator cards of this type exposed to this instance.</rdfs:comment>
    <rdfs:domain rdf:resource="http://example.org/onto/class/google_dataproc_workflow_template"/>
    <rdfs:range rdf:resource="http://www.w3.org/2001/XMLSchema#string"/>
  </owl:DatatypeProperty>
  <owl:DatatypeProperty rdf:about="http://example.org/onto/prop/google_dataproc_workflow_template_accelerator_type">
    <rdfs:label>accelerator_type</rdfs:label>
    <rdfs:comment>Full URL, partial URI, or short name of the accelerator type resource to expose to this instance. See [Compute Engine AcceleratorTypes](https://cloud.google.com/compute/docs/reference/beta/acceleratorTypes). Examples: * `https://www.googleapis.com/compute/beta/projects/[project_id]/zones/us-east1-a/acceleratorTypes/nvidia-tesla-k80` * `projects/[project_id]/zones/us-east1-a/acceleratorTypes/nvidia-tesla-k80` * `nvidia-tesla-k80` **Auto Zone Exception**: If you are using the Dataproc [Auto Zone Placement](https://cloud.google.com/dataproc/docs/concepts/configuring-clusters/auto-zone#using_auto_zone_placement) feature, you must use the short name of the accelerator type resource, for example, `nvidia-tesla-k80`.</rdfs:comment>
    <rdfs:domain rdf:resource="http://example.org/onto/class/google_dataproc_workflow_template"/>
    <rdfs:range rdf:resource="http://www.w3.org/2001/XMLSchema#string"/>
  </owl:DatatypeProperty>
  <owl:DatatypeProperty rdf:about="http://example.org/onto/prop/google_dataproc_workflow_template_boot_disk_size_gb">
    <rdfs:label>boot_disk_size_gb</rdfs:label>
    <rdfs:comment>Optional. Size in GB of the boot disk (default is 500GB).</rdfs:comment>
    <rdfs:domain rdf:resource="http://example.org/onto/class/google_dataproc_workflow_template"/>
    <rdfs:range rdf:resource="http://www.w3.org/2001/XMLSchema#string"/>
  </owl:DatatypeProperty>
  <owl:DatatypeProperty rdf:about="http://example.org/onto/prop/google_dataproc_workflow_template_boot_disk_type">
    <rdfs:label>boot_disk_type</rdfs:label>
    <rdfs:comment>Optional. Type of the boot disk (default is "pd-standard"). Valid values: "pd-balanced" (Persistent Disk Balanced Solid State Drive), "pd-ssd" (Persistent Disk Solid State Drive), or "pd-standard" (Persistent Disk Hard Disk Drive). See [Disk types](https://cloud.google.com/compute/docs/disks#disk-types).</rdfs:comment>
    <rdfs:domain rdf:resource="http://example.org/onto/class/google_dataproc_workflow_template"/>
    <rdfs:range rdf:resource="http://www.w3.org/2001/XMLSchema#string"/>
  </owl:DatatypeProperty>
  <owl:DatatypeProperty rdf:about="http://example.org/onto/prop/google_dataproc_workflow_template_num_local_ssds">
    <rdfs:label>num_local_ssds</rdfs:label>
    <rdfs:comment>Optional. Number of attached SSDs, from 0 to 4 (default is 0). If SSDs are not attached, the boot disk is used to store runtime logs and [HDFS](https://hadoop.apache.org/docs/r1.2.1/hdfs_user_guide.html) data. If one or more SSDs are attached, this runtime bulk data is spread across them, and the boot disk contains only basic config and installed binaries.</rdfs:comment>
    <rdfs:domain rdf:resource="http://example.org/onto/class/google_dataproc_workflow_template"/>
    <rdfs:range rdf:resource="http://www.w3.org/2001/XMLSchema#string"/>
  </owl:DatatypeProperty>
  <owl:DatatypeProperty rdf:about="http://example.org/onto/prop/google_dataproc_workflow_template_create">
    <rdfs:label>create</rdfs:label>
    <rdfs:domain rdf:resource="http://example.org/onto/class/google_dataproc_workflow_template"/>
    <rdfs:range rdf:resource="http://www.w3.org/2001/XMLSchema#string"/>
  </owl:DatatypeProperty>
  <owl:DatatypeProperty rdf:about="http://example.org/onto/prop/google_dataproc_workflow_template_delete">
    <rdfs:label>delete</rdfs:label>
    <rdfs:domain rdf:resource="http://example.org/onto/class/google_dataproc_workflow_template"/>
    <rdfs:range rdf:resource="http://www.w3.org/2001/XMLSchema#string"/>
  </owl:DatatypeProperty>
  <owl:DatatypeProperty rdf:about="http://example.org/onto/prop/google_dataproc_workflow_template_update">
    <rdfs:label>update</rdfs:label>
    <rdfs:domain rdf:resource="http://example.org/onto/class/google_dataproc_workflow_template"/>
    <rdfs:range rdf:resource="http://www.w3.org/2001/XMLSchema#string"/>
  </owl:DatatypeProperty>
</rdf:RDF>
