<?xml version="1.0" encoding="UTF-8"?>
<rdf:RDF
  xmlns:rdf="http://www.w3.org/1999/02/22-rdf-syntax-ns#"
  xmlns:rdfs="http://www.w3.org/2000/01/rdf-schema#"
  xmlns:owl="http://www.w3.org/2002/07/owl#"
  xmlns:xsd="http://www.w3.org/2001/XMLSchema#"
  xml:base="http://example.org/onto/">
  <owl:Class rdf:about="http://example.org/onto/class/google_cloud_run_v2_job">
    <rdfs:label>google_cloud_run_v2_job</rdfs:label>
    <rdfs:comment>#
#     ***     AUTO GENERATED CODE    ***    Type: MMv1     ***
#
# ----------------------------------------------------------------------------
#
#     This code is generated by Magic Modules using the following:
#
#     Configuration: https:#github.com/GoogleCloudPlatform/magic-modules/tree/main/mmv1/products/cloudrunv2/Job.yaml
#     Template:      https:#github.com/GoogleCloudPlatform/magic-modules/tree/main/mmv1/templates/terraform/resource.html.markdown.tmpl
#
#     DO NOT EDIT this file directly. Any changes made to this file will be
#     overwritten during the next generation cycle.
#
# ----------------------------------------------------------------------------
subcategory: "Cloud Run (v2 API)"
description: |-
  A Cloud Run Job resource that references a container image which is run to completion.
---</rdfs:comment>
  </owl:Class>
  <owl:DatatypeProperty rdf:about="http://example.org/onto/prop/google_cloud_run_v2_job_annotations">
    <rdfs:label>annotations</rdfs:label>
    <rdfs:comment>Unstructured key value map that may be set by external tools to store and arbitrary metadata. They are not queryable and should be preserved when modifying objects.

Cloud Run API v2 does not support annotations with 'run.googleapis.com', 'cloud.googleapis.com', 'serving.knative.dev', or 'autoscaling.knative.dev' namespaces, and they will be rejected on new resources.
All system annotations in v1 now have a corresponding field in v2 Job.

This field follows Kubernetes annotations' namespacing, limits, and rules.

**Note**: This field is non-authoritative, and will only manage the annotations present in your configuration.
Please refer to the field 'effective_annotations' for all of the annotations present on the resource.</rdfs:comment>
    <rdfs:domain rdf:resource="http://example.org/onto/class/google_cloud_run_v2_job"/>
    <rdfs:range rdf:resource="http://www.w3.org/2001/XMLSchema#string"/>
  </owl:DatatypeProperty>
  <owl:DatatypeProperty rdf:about="http://example.org/onto/prop/google_cloud_run_v2_job_client">
    <rdfs:label>client</rdfs:label>
    <rdfs:comment>Arbitrary identifier for the API client.</rdfs:comment>
    <rdfs:domain rdf:resource="http://example.org/onto/class/google_cloud_run_v2_job"/>
    <rdfs:range rdf:resource="http://www.w3.org/2001/XMLSchema#string"/>
  </owl:DatatypeProperty>
  <owl:DatatypeProperty rdf:about="http://example.org/onto/prop/google_cloud_run_v2_job_client_version">
    <rdfs:label>client_version</rdfs:label>
    <rdfs:comment>Arbitrary version identifier for the API client.</rdfs:comment>
    <rdfs:domain rdf:resource="http://example.org/onto/class/google_cloud_run_v2_job"/>
    <rdfs:range rdf:resource="http://www.w3.org/2001/XMLSchema#string"/>
  </owl:DatatypeProperty>
  <owl:DatatypeProperty rdf:about="http://example.org/onto/prop/google_cloud_run_v2_job_conditions">
    <rdfs:label>conditions</rdfs:label>
    <rdfs:comment>The Conditions of all other associated sub-resources. They contain additional diagnostics information in case the Job does not reach its desired state. See comments in reconciling for additional information on 'reconciliation' process in Cloud Run.</rdfs:comment>
    <rdfs:domain rdf:resource="http://example.org/onto/class/google_cloud_run_v2_job"/>
    <rdfs:range rdf:resource="http://www.w3.org/2001/XMLSchema#string"/>
  </owl:DatatypeProperty>
  <owl:DatatypeProperty rdf:about="http://example.org/onto/prop/google_cloud_run_v2_job_create_time">
    <rdfs:label>create_time</rdfs:label>
    <rdfs:comment>The creation time.</rdfs:comment>
    <rdfs:domain rdf:resource="http://example.org/onto/class/google_cloud_run_v2_job"/>
    <rdfs:range rdf:resource="http://www.w3.org/2001/XMLSchema#string"/>
  </owl:DatatypeProperty>
  <owl:DatatypeProperty rdf:about="http://example.org/onto/prop/google_cloud_run_v2_job_creator">
    <rdfs:label>creator</rdfs:label>
    <rdfs:comment>Email address of the authenticated creator.</rdfs:comment>
    <rdfs:domain rdf:resource="http://example.org/onto/class/google_cloud_run_v2_job"/>
    <rdfs:range rdf:resource="http://www.w3.org/2001/XMLSchema#string"/>
  </owl:DatatypeProperty>
  <owl:DatatypeProperty rdf:about="http://example.org/onto/prop/google_cloud_run_v2_job_delete_time">
    <rdfs:label>delete_time</rdfs:label>
    <rdfs:comment>The deletion time.</rdfs:comment>
    <rdfs:domain rdf:resource="http://example.org/onto/class/google_cloud_run_v2_job"/>
    <rdfs:range rdf:resource="http://www.w3.org/2001/XMLSchema#string"/>
  </owl:DatatypeProperty>
  <owl:DatatypeProperty rdf:about="http://example.org/onto/prop/google_cloud_run_v2_job_deletion_protection">
    <rdfs:label>deletion_protection</rdfs:label>
    <rdfs:comment>Whether Terraform will be prevented from destroying the job. Defaults to true.
When a'terraform destroy' or 'terraform apply' would delete the job,
the command will fail if this field is not set to false in Terraform state.
When the field is set to true or unset in Terraform state, a 'terraform apply'
or 'terraform destroy' that would delete the job will fail.
When the field is set to false, deleting the job is allowed.</rdfs:comment>
    <rdfs:domain rdf:resource="http://example.org/onto/class/google_cloud_run_v2_job"/>
    <rdfs:range rdf:resource="http://www.w3.org/2001/XMLSchema#string"/>
  </owl:DatatypeProperty>
  <owl:DatatypeProperty rdf:about="http://example.org/onto/prop/google_cloud_run_v2_job_effective_annotations">
    <rdfs:label>effective_annotations</rdfs:label>
    <rdfs:comment>All of annotations (key/value pairs) present on the resource in GCP, including the annotations configured through Terraform, other clients and services.</rdfs:comment>
    <rdfs:domain rdf:resource="http://example.org/onto/class/google_cloud_run_v2_job"/>
    <rdfs:range rdf:resource="http://www.w3.org/2001/XMLSchema#string"/>
  </owl:DatatypeProperty>
  <owl:DatatypeProperty rdf:about="http://example.org/onto/prop/google_cloud_run_v2_job_effective_labels">
    <rdfs:label>effective_labels</rdfs:label>
    <rdfs:comment>All of labels (key/value pairs) present on the resource in GCP, including the labels configured through Terraform, other clients and services.</rdfs:comment>
    <rdfs:domain rdf:resource="http://example.org/onto/class/google_cloud_run_v2_job"/>
    <rdfs:range rdf:resource="http://www.w3.org/2001/XMLSchema#string"/>
  </owl:DatatypeProperty>
  <owl:DatatypeProperty rdf:about="http://example.org/onto/prop/google_cloud_run_v2_job_etag">
    <rdfs:label>etag</rdfs:label>
    <rdfs:comment>A system-generated fingerprint for this version of the resource. May be used to detect modification conflict during updates.</rdfs:comment>
    <rdfs:domain rdf:resource="http://example.org/onto/class/google_cloud_run_v2_job"/>
    <rdfs:range rdf:resource="http://www.w3.org/2001/XMLSchema#string"/>
  </owl:DatatypeProperty>
  <owl:DatatypeProperty rdf:about="http://example.org/onto/prop/google_cloud_run_v2_job_execution_count">
    <rdfs:label>execution_count</rdfs:label>
    <rdfs:comment>Number of executions created for this job.</rdfs:comment>
    <rdfs:domain rdf:resource="http://example.org/onto/class/google_cloud_run_v2_job"/>
    <rdfs:range rdf:resource="http://www.w3.org/2001/XMLSchema#string"/>
  </owl:DatatypeProperty>
  <owl:DatatypeProperty rdf:about="http://example.org/onto/prop/google_cloud_run_v2_job_expire_time">
    <rdfs:label>expire_time</rdfs:label>
    <rdfs:comment>For a deleted resource, the time after which it will be permanently deleted.</rdfs:comment>
    <rdfs:domain rdf:resource="http://example.org/onto/class/google_cloud_run_v2_job"/>
    <rdfs:range rdf:resource="http://www.w3.org/2001/XMLSchema#string"/>
  </owl:DatatypeProperty>
  <owl:DatatypeProperty rdf:about="http://example.org/onto/prop/google_cloud_run_v2_job_generation">
    <rdfs:label>generation</rdfs:label>
    <rdfs:comment>A number that monotonically increases every time the user modifies the desired state.</rdfs:comment>
    <rdfs:domain rdf:resource="http://example.org/onto/class/google_cloud_run_v2_job"/>
    <rdfs:range rdf:resource="http://www.w3.org/2001/XMLSchema#string"/>
  </owl:DatatypeProperty>
  <owl:DatatypeProperty rdf:about="http://example.org/onto/prop/google_cloud_run_v2_job_id">
    <rdfs:label>id</rdfs:label>
    <rdfs:domain rdf:resource="http://example.org/onto/class/google_cloud_run_v2_job"/>
    <rdfs:range rdf:resource="http://www.w3.org/2001/XMLSchema#string"/>
  </owl:DatatypeProperty>
  <owl:DatatypeProperty rdf:about="http://example.org/onto/prop/google_cloud_run_v2_job_labels">
    <rdfs:label>labels</rdfs:label>
    <rdfs:comment>Unstructured key value map that can be used to organize and categorize objects. User-provided labels are shared with Google's billing system, so they can be used to filter, or break down billing charges by team, component,
environment, state, etc. For more information, visit https://cloud.google.com/resource-manager/docs/creating-managing-labels or https://cloud.google.com/run/docs/configuring/labels.

Cloud Run API v2 does not support labels with 'run.googleapis.com', 'cloud.googleapis.com', 'serving.knative.dev', or 'autoscaling.knative.dev' namespaces, and they will be rejected.
All system labels in v1 now have a corresponding field in v2 Job.

**Note**: This field is non-authoritative, and will only manage the labels present in your configuration.
Please refer to the field 'effective_labels' for all of the labels present on the resource.</rdfs:comment>
    <rdfs:domain rdf:resource="http://example.org/onto/class/google_cloud_run_v2_job"/>
    <rdfs:range rdf:resource="http://www.w3.org/2001/XMLSchema#string"/>
  </owl:DatatypeProperty>
  <owl:DatatypeProperty rdf:about="http://example.org/onto/prop/google_cloud_run_v2_job_last_modifier">
    <rdfs:label>last_modifier</rdfs:label>
    <rdfs:comment>Email address of the last authenticated modifier.</rdfs:comment>
    <rdfs:domain rdf:resource="http://example.org/onto/class/google_cloud_run_v2_job"/>
    <rdfs:range rdf:resource="http://www.w3.org/2001/XMLSchema#string"/>
  </owl:DatatypeProperty>
  <owl:DatatypeProperty rdf:about="http://example.org/onto/prop/google_cloud_run_v2_job_latest_created_execution">
    <rdfs:label>latest_created_execution</rdfs:label>
    <rdfs:comment>Name of the last created execution.</rdfs:comment>
    <rdfs:domain rdf:resource="http://example.org/onto/class/google_cloud_run_v2_job"/>
    <rdfs:range rdf:resource="http://www.w3.org/2001/XMLSchema#string"/>
  </owl:DatatypeProperty>
  <owl:DatatypeProperty rdf:about="http://example.org/onto/prop/google_cloud_run_v2_job_launch_stage">
    <rdfs:label>launch_stage</rdfs:label>
    <rdfs:comment>The launch stage as defined by [Google Cloud Platform Launch Stages](https://cloud.google.com/products#product-launch-stages). Cloud Run supports ALPHA, BETA, and GA.
If no value is specified, GA is assumed. Set the launch stage to a preview stage on input to allow use of preview features in that stage. On read (or output), describes whether the resource uses preview features.

For example, if ALPHA is provided as input, but only BETA and GA-level features are used, this field will be BETA on output. Possible values: ["UNIMPLEMENTED", "PRELAUNCH", "EARLY_ACCESS", "ALPHA", "BETA", "GA", "DEPRECATED"]</rdfs:comment>
    <rdfs:domain rdf:resource="http://example.org/onto/class/google_cloud_run_v2_job"/>
    <rdfs:range rdf:resource="http://www.w3.org/2001/XMLSchema#string"/>
  </owl:DatatypeProperty>
  <owl:DatatypeProperty rdf:about="http://example.org/onto/prop/google_cloud_run_v2_job_location">
    <rdfs:label>location</rdfs:label>
    <rdfs:comment>The location of the cloud run job</rdfs:comment>
    <rdfs:domain rdf:resource="http://example.org/onto/class/google_cloud_run_v2_job"/>
    <rdfs:range rdf:resource="http://www.w3.org/2001/XMLSchema#string"/>
  </owl:DatatypeProperty>
  <owl:DatatypeProperty rdf:about="http://example.org/onto/prop/google_cloud_run_v2_job_name">
    <rdfs:label>name</rdfs:label>
    <rdfs:comment>Name of the Job.</rdfs:comment>
    <rdfs:domain rdf:resource="http://example.org/onto/class/google_cloud_run_v2_job"/>
    <rdfs:range rdf:resource="http://www.w3.org/2001/XMLSchema#string"/>
  </owl:DatatypeProperty>
  <owl:DatatypeProperty rdf:about="http://example.org/onto/prop/google_cloud_run_v2_job_observed_generation">
    <rdfs:label>observed_generation</rdfs:label>
    <rdfs:comment>The generation of this Job. See comments in reconciling for additional information on reconciliation process in Cloud Run.</rdfs:comment>
    <rdfs:domain rdf:resource="http://example.org/onto/class/google_cloud_run_v2_job"/>
    <rdfs:range rdf:resource="http://www.w3.org/2001/XMLSchema#string"/>
  </owl:DatatypeProperty>
  <owl:DatatypeProperty rdf:about="http://example.org/onto/prop/google_cloud_run_v2_job_project">
    <rdfs:label>project</rdfs:label>
    <rdfs:domain rdf:resource="http://example.org/onto/class/google_cloud_run_v2_job"/>
    <rdfs:range rdf:resource="http://www.w3.org/2001/XMLSchema#string"/>
  </owl:DatatypeProperty>
  <owl:DatatypeProperty rdf:about="http://example.org/onto/prop/google_cloud_run_v2_job_reconciling">
    <rdfs:label>reconciling</rdfs:label>
    <rdfs:comment>Returns true if the Job is currently being acted upon by the system to bring it into the desired state.

When a new Job is created, or an existing one is updated, Cloud Run will asynchronously perform all necessary steps to bring the Job to the desired state. This process is called reconciliation. While reconciliation is in process, observedGeneration and latest_succeeded_execution, will have transient values that might mismatch the intended state: Once reconciliation is over (and this field is false), there are two possible outcomes: reconciliation succeeded and the state matches the Job, or there was an error, and reconciliation failed. This state can be found in terminalCondition.state.

If reconciliation succeeded, the following fields will match: observedGeneration and generation, latest_succeeded_execution and latestCreatedExecution.

If reconciliation failed, observedGeneration and latest_succeeded_execution will have the state of the last succeeded execution or empty for newly created Job. Additional information on the failure can be found in terminalCondition and conditions</rdfs:comment>
    <rdfs:domain rdf:resource="http://example.org/onto/class/google_cloud_run_v2_job"/>
    <rdfs:range rdf:resource="http://www.w3.org/2001/XMLSchema#string"/>
  </owl:DatatypeProperty>
  <owl:DatatypeProperty rdf:about="http://example.org/onto/prop/google_cloud_run_v2_job_terminal_condition">
    <rdfs:label>terminal_condition</rdfs:label>
    <rdfs:comment>The Condition of this Job, containing its readiness status, and detailed error information in case it did not reach the desired state</rdfs:comment>
    <rdfs:domain rdf:resource="http://example.org/onto/class/google_cloud_run_v2_job"/>
    <rdfs:range rdf:resource="http://www.w3.org/2001/XMLSchema#string"/>
  </owl:DatatypeProperty>
  <owl:DatatypeProperty rdf:about="http://example.org/onto/prop/google_cloud_run_v2_job_terraform_labels">
    <rdfs:label>terraform_labels</rdfs:label>
    <rdfs:comment>The combination of labels configured directly on the resource
 and default labels configured on the provider.</rdfs:comment>
    <rdfs:domain rdf:resource="http://example.org/onto/class/google_cloud_run_v2_job"/>
    <rdfs:range rdf:resource="http://www.w3.org/2001/XMLSchema#string"/>
  </owl:DatatypeProperty>
  <owl:DatatypeProperty rdf:about="http://example.org/onto/prop/google_cloud_run_v2_job_uid">
    <rdfs:label>uid</rdfs:label>
    <rdfs:comment>Server assigned unique identifier for the Execution. The value is a UUID4 string and guaranteed to remain unchanged until the resource is deleted.</rdfs:comment>
    <rdfs:domain rdf:resource="http://example.org/onto/class/google_cloud_run_v2_job"/>
    <rdfs:range rdf:resource="http://www.w3.org/2001/XMLSchema#string"/>
  </owl:DatatypeProperty>
  <owl:DatatypeProperty rdf:about="http://example.org/onto/prop/google_cloud_run_v2_job_update_time">
    <rdfs:label>update_time</rdfs:label>
    <rdfs:comment>The last-modified time.</rdfs:comment>
    <rdfs:domain rdf:resource="http://example.org/onto/class/google_cloud_run_v2_job"/>
    <rdfs:range rdf:resource="http://www.w3.org/2001/XMLSchema#string"/>
  </owl:DatatypeProperty>
  <owl:DatatypeProperty rdf:about="http://example.org/onto/prop/google_cloud_run_v2_job_breakglass_justification">
    <rdfs:label>breakglass_justification</rdfs:label>
    <rdfs:comment>If present, indicates to use Breakglass using this justification. If useDefault is False, then it must be empty. For more information on breakglass, see https://cloud.google.com/binary-authorization/docs/using-breakglass</rdfs:comment>
    <rdfs:domain rdf:resource="http://example.org/onto/class/google_cloud_run_v2_job"/>
    <rdfs:range rdf:resource="http://www.w3.org/2001/XMLSchema#string"/>
  </owl:DatatypeProperty>
  <owl:DatatypeProperty rdf:about="http://example.org/onto/prop/google_cloud_run_v2_job_policy">
    <rdfs:label>policy</rdfs:label>
    <rdfs:comment>The path to a binary authorization policy. Format: projects/{project}/platforms/cloudRun/{policy-name}</rdfs:comment>
    <rdfs:domain rdf:resource="http://example.org/onto/class/google_cloud_run_v2_job"/>
    <rdfs:range rdf:resource="http://www.w3.org/2001/XMLSchema#string"/>
  </owl:DatatypeProperty>
  <owl:DatatypeProperty rdf:about="http://example.org/onto/prop/google_cloud_run_v2_job_use_default">
    <rdfs:label>use_default</rdfs:label>
    <rdfs:comment>If True, indicates to use the default project's binary authorization policy. If False, binary authorization will be disabled.</rdfs:comment>
    <rdfs:domain rdf:resource="http://example.org/onto/class/google_cloud_run_v2_job"/>
    <rdfs:range rdf:resource="http://www.w3.org/2001/XMLSchema#string"/>
  </owl:DatatypeProperty>
  <owl:DatatypeProperty rdf:about="http://example.org/onto/prop/google_cloud_run_v2_job_annotations">
    <rdfs:label>annotations</rdfs:label>
    <rdfs:comment>Unstructured key value map that may be set by external tools to store and arbitrary metadata. They are not queryable and should be preserved when modifying objects.

Cloud Run API v2 does not support annotations with 'run.googleapis.com', 'cloud.googleapis.com', 'serving.knative.dev', or 'autoscaling.knative.dev' namespaces, and they will be rejected.
All system annotations in v1 now have a corresponding field in v2 ExecutionTemplate.

This field follows Kubernetes annotations' namespacing, limits, and rules.</rdfs:comment>
    <rdfs:domain rdf:resource="http://example.org/onto/class/google_cloud_run_v2_job"/>
    <rdfs:range rdf:resource="http://www.w3.org/2001/XMLSchema#string"/>
  </owl:DatatypeProperty>
  <owl:DatatypeProperty rdf:about="http://example.org/onto/prop/google_cloud_run_v2_job_labels">
    <rdfs:label>labels</rdfs:label>
    <rdfs:comment>Unstructured key value map that can be used to organize and categorize objects. User-provided labels are shared with Google's billing system, so they can be used to filter,
or break down billing charges by team, component, environment, state, etc. For more information, visit https://cloud.google.com/resource-manager/docs/creating-managing-labels or
https://cloud.google.com/run/docs/configuring/labels.

Cloud Run API v2 does not support labels with 'run.googleapis.com', 'cloud.googleapis.com', 'serving.knative.dev', or 'autoscaling.knative.dev' namespaces, and they will be rejected.
All system labels in v1 now have a corresponding field in v2 ExecutionTemplate.</rdfs:comment>
    <rdfs:domain rdf:resource="http://example.org/onto/class/google_cloud_run_v2_job"/>
    <rdfs:range rdf:resource="http://www.w3.org/2001/XMLSchema#string"/>
  </owl:DatatypeProperty>
  <owl:DatatypeProperty rdf:about="http://example.org/onto/prop/google_cloud_run_v2_job_parallelism">
    <rdfs:label>parallelism</rdfs:label>
    <rdfs:comment>Specifies the maximum desired number of tasks the execution should run at given time. Must be <= taskCount. When the job is run, if this field is 0 or unset, the maximum possible value will be used for that execution. The actual number of tasks running in steady state will be less than this number when there are fewer tasks waiting to be completed remaining, i.e. when the work left to do is less than max parallelism.</rdfs:comment>
    <rdfs:domain rdf:resource="http://example.org/onto/class/google_cloud_run_v2_job"/>
    <rdfs:range rdf:resource="http://www.w3.org/2001/XMLSchema#string"/>
  </owl:DatatypeProperty>
  <owl:DatatypeProperty rdf:about="http://example.org/onto/prop/google_cloud_run_v2_job_task_count">
    <rdfs:label>task_count</rdfs:label>
    <rdfs:comment>Specifies the desired number of tasks the execution should run. Setting to 1 means that parallelism is limited to 1 and the success of that task signals the success of the execution. More info: https://kubernetes.io/docs/concepts/workloads/controllers/jobs-run-to-completion/</rdfs:comment>
    <rdfs:domain rdf:resource="http://example.org/onto/class/google_cloud_run_v2_job"/>
    <rdfs:range rdf:resource="http://www.w3.org/2001/XMLSchema#string"/>
  </owl:DatatypeProperty>
  <owl:DatatypeProperty rdf:about="http://example.org/onto/prop/google_cloud_run_v2_job_encryption_key">
    <rdfs:label>encryption_key</rdfs:label>
    <rdfs:comment>A reference to a customer managed encryption key (CMEK) to use to encrypt this container image. For more information, go to https://cloud.google.com/run/docs/securing/using-cmek</rdfs:comment>
    <rdfs:domain rdf:resource="http://example.org/onto/class/google_cloud_run_v2_job"/>
    <rdfs:range rdf:resource="http://www.w3.org/2001/XMLSchema#string"/>
  </owl:DatatypeProperty>
  <owl:DatatypeProperty rdf:about="http://example.org/onto/prop/google_cloud_run_v2_job_execution_environment">
    <rdfs:label>execution_environment</rdfs:label>
    <rdfs:comment>The execution environment being used to host this Task. Possible values: ["EXECUTION_ENVIRONMENT_GEN1", "EXECUTION_ENVIRONMENT_GEN2"]</rdfs:comment>
    <rdfs:domain rdf:resource="http://example.org/onto/class/google_cloud_run_v2_job"/>
    <rdfs:range rdf:resource="http://www.w3.org/2001/XMLSchema#string"/>
  </owl:DatatypeProperty>
  <owl:DatatypeProperty rdf:about="http://example.org/onto/prop/google_cloud_run_v2_job_gpu_zonal_redundancy_disabled">
    <rdfs:label>gpu_zonal_redundancy_disabled</rdfs:label>
    <rdfs:comment>True if GPU zonal redundancy is disabled on this execution.</rdfs:comment>
    <rdfs:domain rdf:resource="http://example.org/onto/class/google_cloud_run_v2_job"/>
    <rdfs:range rdf:resource="http://www.w3.org/2001/XMLSchema#string"/>
  </owl:DatatypeProperty>
  <owl:DatatypeProperty rdf:about="http://example.org/onto/prop/google_cloud_run_v2_job_max_retries">
    <rdfs:label>max_retries</rdfs:label>
    <rdfs:comment>Number of retries allowed per Task, before marking this Task failed. Defaults to 3. Minimum value is 0.</rdfs:comment>
    <rdfs:domain rdf:resource="http://example.org/onto/class/google_cloud_run_v2_job"/>
    <rdfs:range rdf:resource="http://www.w3.org/2001/XMLSchema#string"/>
  </owl:DatatypeProperty>
  <owl:DatatypeProperty rdf:about="http://example.org/onto/prop/google_cloud_run_v2_job_service_account">
    <rdfs:label>service_account</rdfs:label>
    <rdfs:comment>Email address of the IAM service account associated with the Task of a Job. The service account represents the identity of the running task, and determines what permissions the task has. If not provided, the task will use the project's default service account.</rdfs:comment>
    <rdfs:domain rdf:resource="http://example.org/onto/class/google_cloud_run_v2_job"/>
    <rdfs:range rdf:resource="http://www.w3.org/2001/XMLSchema#string"/>
  </owl:DatatypeProperty>
  <owl:DatatypeProperty rdf:about="http://example.org/onto/prop/google_cloud_run_v2_job_timeout">
    <rdfs:label>timeout</rdfs:label>
    <rdfs:comment>Max allowed time duration the Task may be active before the system will actively try to mark it failed and kill associated containers. This applies per attempt of a task, meaning each retry can run for the full timeout.

A duration in seconds with up to nine fractional digits, ending with 's'. Example: "3.5s".</rdfs:comment>
    <rdfs:domain rdf:resource="http://example.org/onto/class/google_cloud_run_v2_job"/>
    <rdfs:range rdf:resource="http://www.w3.org/2001/XMLSchema#string"/>
  </owl:DatatypeProperty>
  <owl:DatatypeProperty rdf:about="http://example.org/onto/prop/google_cloud_run_v2_job_args">
    <rdfs:label>args</rdfs:label>
    <rdfs:comment>Arguments to the entrypoint. The docker image's CMD is used if this is not provided. Variable references are not supported in Cloud Run.</rdfs:comment>
    <rdfs:domain rdf:resource="http://example.org/onto/class/google_cloud_run_v2_job"/>
    <rdfs:range rdf:resource="http://www.w3.org/2001/XMLSchema#string"/>
  </owl:DatatypeProperty>
  <owl:DatatypeProperty rdf:about="http://example.org/onto/prop/google_cloud_run_v2_job_command">
    <rdfs:label>command</rdfs:label>
    <rdfs:comment>Entrypoint array. Not executed within a shell. The docker image's ENTRYPOINT is used if this is not provided. Variable references $(VAR_NAME) are expanded using the container's environment. If a variable cannot be resolved, the reference in the input string will be unchanged. The $(VAR_NAME) syntax can be escaped with a double $$, ie: $$(VAR_NAME). Escaped references will never be expanded, regardless of whether the variable exists or not. More info: https://kubernetes.io/docs/tasks/inject-data-application/define-command-argument-container/#running-a-command-in-a-shell</rdfs:comment>
    <rdfs:domain rdf:resource="http://example.org/onto/class/google_cloud_run_v2_job"/>
    <rdfs:range rdf:resource="http://www.w3.org/2001/XMLSchema#string"/>
  </owl:DatatypeProperty>
  <owl:DatatypeProperty rdf:about="http://example.org/onto/prop/google_cloud_run_v2_job_depends_on">
    <rdfs:label>depends_on</rdfs:label>
    <rdfs:comment>Names of the containers that must start before this container.</rdfs:comment>
    <rdfs:domain rdf:resource="http://example.org/onto/class/google_cloud_run_v2_job"/>
    <rdfs:range rdf:resource="http://www.w3.org/2001/XMLSchema#string"/>
  </owl:DatatypeProperty>
  <owl:DatatypeProperty rdf:about="http://example.org/onto/prop/google_cloud_run_v2_job_image">
    <rdfs:label>image</rdfs:label>
    <rdfs:comment>URL of the Container image in Google Container Registry or Google Artifact Registry. More info: https://kubernetes.io/docs/concepts/containers/images</rdfs:comment>
    <rdfs:domain rdf:resource="http://example.org/onto/class/google_cloud_run_v2_job"/>
    <rdfs:range rdf:resource="http://www.w3.org/2001/XMLSchema#string"/>
  </owl:DatatypeProperty>
  <owl:DatatypeProperty rdf:about="http://example.org/onto/prop/google_cloud_run_v2_job_name">
    <rdfs:label>name</rdfs:label>
    <rdfs:comment>Name of the container specified as a DNS_LABEL.</rdfs:comment>
    <rdfs:domain rdf:resource="http://example.org/onto/class/google_cloud_run_v2_job"/>
    <rdfs:range rdf:resource="http://www.w3.org/2001/XMLSchema#string"/>
  </owl:DatatypeProperty>
  <owl:DatatypeProperty rdf:about="http://example.org/onto/prop/google_cloud_run_v2_job_working_dir">
    <rdfs:label>working_dir</rdfs:label>
    <rdfs:comment>Container's working directory. If not specified, the container runtime's default will be used, which might be configured in the container image.</rdfs:comment>
    <rdfs:domain rdf:resource="http://example.org/onto/class/google_cloud_run_v2_job"/>
    <rdfs:range rdf:resource="http://www.w3.org/2001/XMLSchema#string"/>
  </owl:DatatypeProperty>
  <owl:DatatypeProperty rdf:about="http://example.org/onto/prop/google_cloud_run_v2_job_name">
    <rdfs:label>name</rdfs:label>
    <rdfs:comment>Name of the environment variable. Must be a C_IDENTIFIER, and mnay not exceed 32768 characters.</rdfs:comment>
    <rdfs:domain rdf:resource="http://example.org/onto/class/google_cloud_run_v2_job"/>
    <rdfs:range rdf:resource="http://www.w3.org/2001/XMLSchema#string"/>
  </owl:DatatypeProperty>
  <owl:DatatypeProperty rdf:about="http://example.org/onto/prop/google_cloud_run_v2_job_value">
    <rdfs:label>value</rdfs:label>
    <rdfs:comment>Literal value of the environment variable. Defaults to "" and the maximum allowed length is 32768 characters. Variable references are not supported in Cloud Run.</rdfs:comment>
    <rdfs:domain rdf:resource="http://example.org/onto/class/google_cloud_run_v2_job"/>
    <rdfs:range rdf:resource="http://www.w3.org/2001/XMLSchema#string"/>
  </owl:DatatypeProperty>
  <owl:DatatypeProperty rdf:about="http://example.org/onto/prop/google_cloud_run_v2_job_secret">
    <rdfs:label>secret</rdfs:label>
    <rdfs:comment>The name of the secret in Cloud Secret Manager. Format: {secretName} if the secret is in the same project. projects/{project}/secrets/{secretName} if the secret is in a different project.</rdfs:comment>
    <rdfs:domain rdf:resource="http://example.org/onto/class/google_cloud_run_v2_job"/>
    <rdfs:range rdf:resource="http://www.w3.org/2001/XMLSchema#string"/>
  </owl:DatatypeProperty>
  <owl:DatatypeProperty rdf:about="http://example.org/onto/prop/google_cloud_run_v2_job_version">
    <rdfs:label>version</rdfs:label>
    <rdfs:comment>The Cloud Secret Manager secret version. Can be 'latest' for the latest value or an integer for a specific version.</rdfs:comment>
    <rdfs:domain rdf:resource="http://example.org/onto/class/google_cloud_run_v2_job"/>
    <rdfs:range rdf:resource="http://www.w3.org/2001/XMLSchema#string"/>
  </owl:DatatypeProperty>
  <owl:DatatypeProperty rdf:about="http://example.org/onto/prop/google_cloud_run_v2_job_container_port">
    <rdfs:label>container_port</rdfs:label>
    <rdfs:comment>Port number the container listens on. This must be a valid TCP port number, 0 < containerPort < 65536.</rdfs:comment>
    <rdfs:domain rdf:resource="http://example.org/onto/class/google_cloud_run_v2_job"/>
    <rdfs:range rdf:resource="http://www.w3.org/2001/XMLSchema#string"/>
  </owl:DatatypeProperty>
  <owl:DatatypeProperty rdf:about="http://example.org/onto/prop/google_cloud_run_v2_job_name">
    <rdfs:label>name</rdfs:label>
    <rdfs:comment>If specified, used to specify which protocol to use. Allowed values are "http1" and "h2c".</rdfs:comment>
    <rdfs:domain rdf:resource="http://example.org/onto/class/google_cloud_run_v2_job"/>
    <rdfs:range rdf:resource="http://www.w3.org/2001/XMLSchema#string"/>
  </owl:DatatypeProperty>
  <owl:DatatypeProperty rdf:about="http://example.org/onto/prop/google_cloud_run_v2_job_limits">
    <rdfs:label>limits</rdfs:label>
    <rdfs:comment>Only memory, CPU, and nvidia.com/gpu are supported. Use key 'cpu' for CPU limit, 'memory' for memory limit, 'nvidia.com/gpu' for gpu limit. Note: The only supported values for CPU are '1', '2', '4', and '8'. Setting 4 CPU requires at least 2Gi of memory. The values of the map is string form of the 'quantity' k8s type: https://github.com/kubernetes/kubernetes/blob/master/staging/src/k8s.io/apimachinery/pkg/api/resource/quantity.go</rdfs:comment>
    <rdfs:domain rdf:resource="http://example.org/onto/class/google_cloud_run_v2_job"/>
    <rdfs:range rdf:resource="http://www.w3.org/2001/XMLSchema#string"/>
  </owl:DatatypeProperty>
  <owl:DatatypeProperty rdf:about="http://example.org/onto/prop/google_cloud_run_v2_job_failure_threshold">
    <rdfs:label>failure_threshold</rdfs:label>
    <rdfs:comment>Minimum consecutive failures for the probe to be considered failed after
having succeeded. Defaults to 3. Minimum value is 1.</rdfs:comment>
    <rdfs:domain rdf:resource="http://example.org/onto/class/google_cloud_run_v2_job"/>
    <rdfs:range rdf:resource="http://www.w3.org/2001/XMLSchema#string"/>
  </owl:DatatypeProperty>
  <owl:DatatypeProperty rdf:about="http://example.org/onto/prop/google_cloud_run_v2_job_initial_delay_seconds">
    <rdfs:label>initial_delay_seconds</rdfs:label>
    <rdfs:comment>Number of seconds after the container has started before the probe is
initiated.
Defaults to 0 seconds. Minimum value is 0. Maximum value is 240.</rdfs:comment>
    <rdfs:domain rdf:resource="http://example.org/onto/class/google_cloud_run_v2_job"/>
    <rdfs:range rdf:resource="http://www.w3.org/2001/XMLSchema#string"/>
  </owl:DatatypeProperty>
  <owl:DatatypeProperty rdf:about="http://example.org/onto/prop/google_cloud_run_v2_job_period_seconds">
    <rdfs:label>period_seconds</rdfs:label>
    <rdfs:comment>How often (in seconds) to perform the probe.
Default to 10 seconds. Minimum value is 1. Maximum value is 240.</rdfs:comment>
    <rdfs:domain rdf:resource="http://example.org/onto/class/google_cloud_run_v2_job"/>
    <rdfs:range rdf:resource="http://www.w3.org/2001/XMLSchema#string"/>
  </owl:DatatypeProperty>
  <owl:DatatypeProperty rdf:about="http://example.org/onto/prop/google_cloud_run_v2_job_timeout_seconds">
    <rdfs:label>timeout_seconds</rdfs:label>
    <rdfs:comment>Number of seconds after which the probe times out.
Defaults to 1 second. Minimum value is 1. Maximum value is 3600.
Must be smaller than periodSeconds.</rdfs:comment>
    <rdfs:domain rdf:resource="http://example.org/onto/class/google_cloud_run_v2_job"/>
    <rdfs:range rdf:resource="http://www.w3.org/2001/XMLSchema#string"/>
  </owl:DatatypeProperty>
  <owl:DatatypeProperty rdf:about="http://example.org/onto/prop/google_cloud_run_v2_job_port">
    <rdfs:label>port</rdfs:label>
    <rdfs:comment>Port number to access on the container. Number must be in the range 1 to 65535.
If not specified, defaults to the same value as container.ports[0].containerPort.</rdfs:comment>
    <rdfs:domain rdf:resource="http://example.org/onto/class/google_cloud_run_v2_job"/>
    <rdfs:range rdf:resource="http://www.w3.org/2001/XMLSchema#string"/>
  </owl:DatatypeProperty>
  <owl:DatatypeProperty rdf:about="http://example.org/onto/prop/google_cloud_run_v2_job_service">
    <rdfs:label>service</rdfs:label>
    <rdfs:comment>The name of the service to place in the gRPC HealthCheckRequest
(see https://github.com/grpc/grpc/blob/master/doc/health-checking.md).
If this is not specified, the default behavior is defined by gRPC.</rdfs:comment>
    <rdfs:domain rdf:resource="http://example.org/onto/class/google_cloud_run_v2_job"/>
    <rdfs:range rdf:resource="http://www.w3.org/2001/XMLSchema#string"/>
  </owl:DatatypeProperty>
  <owl:DatatypeProperty rdf:about="http://example.org/onto/prop/google_cloud_run_v2_job_path">
    <rdfs:label>path</rdfs:label>
    <rdfs:comment>Path to access on the HTTP server. If set, it should not be empty string.</rdfs:comment>
    <rdfs:domain rdf:resource="http://example.org/onto/class/google_cloud_run_v2_job"/>
    <rdfs:range rdf:resource="http://www.w3.org/2001/XMLSchema#string"/>
  </owl:DatatypeProperty>
  <owl:DatatypeProperty rdf:about="http://example.org/onto/prop/google_cloud_run_v2_job_port">
    <rdfs:label>port</rdfs:label>
    <rdfs:comment>Port number to access on the container. Number must be in the range 1 to 65535.
If not specified, defaults to the same value as container.ports[0].containerPort.</rdfs:comment>
    <rdfs:domain rdf:resource="http://example.org/onto/class/google_cloud_run_v2_job"/>
    <rdfs:range rdf:resource="http://www.w3.org/2001/XMLSchema#string"/>
  </owl:DatatypeProperty>
  <owl:DatatypeProperty rdf:about="http://example.org/onto/prop/google_cloud_run_v2_job_name">
    <rdfs:label>name</rdfs:label>
    <rdfs:comment>The header field name.</rdfs:comment>
    <rdfs:domain rdf:resource="http://example.org/onto/class/google_cloud_run_v2_job"/>
    <rdfs:range rdf:resource="http://www.w3.org/2001/XMLSchema#string"/>
  </owl:DatatypeProperty>
  <owl:DatatypeProperty rdf:about="http://example.org/onto/prop/google_cloud_run_v2_job_value">
    <rdfs:label>value</rdfs:label>
    <rdfs:comment>The header field value.</rdfs:comment>
    <rdfs:domain rdf:resource="http://example.org/onto/class/google_cloud_run_v2_job"/>
    <rdfs:range rdf:resource="http://www.w3.org/2001/XMLSchema#string"/>
  </owl:DatatypeProperty>
  <owl:DatatypeProperty rdf:about="http://example.org/onto/prop/google_cloud_run_v2_job_port">
    <rdfs:label>port</rdfs:label>
    <rdfs:comment>Port number to access on the container. Number must be in the range 1 to 65535.
If not specified, defaults to the same value as container.ports[0].containerPort.</rdfs:comment>
    <rdfs:domain rdf:resource="http://example.org/onto/class/google_cloud_run_v2_job"/>
    <rdfs:range rdf:resource="http://www.w3.org/2001/XMLSchema#string"/>
  </owl:DatatypeProperty>
  <owl:DatatypeProperty rdf:about="http://example.org/onto/prop/google_cloud_run_v2_job_mount_path">
    <rdfs:label>mount_path</rdfs:label>
    <rdfs:comment>Path within the container at which the volume should be mounted. Must not contain ':'. For Cloud SQL volumes, it can be left empty, or must otherwise be /cloudsql. All instances defined in the Volume will be available as /cloudsql/[instance]. For more information on Cloud SQL volumes, visit https://cloud.google.com/sql/docs/mysql/connect-run</rdfs:comment>
    <rdfs:domain rdf:resource="http://example.org/onto/class/google_cloud_run_v2_job"/>
    <rdfs:range rdf:resource="http://www.w3.org/2001/XMLSchema#string"/>
  </owl:DatatypeProperty>
  <owl:DatatypeProperty rdf:about="http://example.org/onto/prop/google_cloud_run_v2_job_name">
    <rdfs:label>name</rdfs:label>
    <rdfs:comment>This must match the Name of a Volume.</rdfs:comment>
    <rdfs:domain rdf:resource="http://example.org/onto/class/google_cloud_run_v2_job"/>
    <rdfs:range rdf:resource="http://www.w3.org/2001/XMLSchema#string"/>
  </owl:DatatypeProperty>
  <owl:DatatypeProperty rdf:about="http://example.org/onto/prop/google_cloud_run_v2_job_sub_path">
    <rdfs:label>sub_path</rdfs:label>
    <rdfs:comment>Path within the volume from which the container's volume should be mounted.</rdfs:comment>
    <rdfs:domain rdf:resource="http://example.org/onto/class/google_cloud_run_v2_job"/>
    <rdfs:range rdf:resource="http://www.w3.org/2001/XMLSchema#string"/>
  </owl:DatatypeProperty>
  <owl:DatatypeProperty rdf:about="http://example.org/onto/prop/google_cloud_run_v2_job_accelerator">
    <rdfs:label>accelerator</rdfs:label>
    <rdfs:comment>The GPU to attach to an instance. See https://cloud.google.com/run/docs/configuring/jobs/gpu for configuring GPU.</rdfs:comment>
    <rdfs:domain rdf:resource="http://example.org/onto/class/google_cloud_run_v2_job"/>
    <rdfs:range rdf:resource="http://www.w3.org/2001/XMLSchema#string"/>
  </owl:DatatypeProperty>
  <owl:DatatypeProperty rdf:about="http://example.org/onto/prop/google_cloud_run_v2_job_name">
    <rdfs:label>name</rdfs:label>
    <rdfs:comment>Volume's name.</rdfs:comment>
    <rdfs:domain rdf:resource="http://example.org/onto/class/google_cloud_run_v2_job"/>
    <rdfs:range rdf:resource="http://www.w3.org/2001/XMLSchema#string"/>
  </owl:DatatypeProperty>
  <owl:DatatypeProperty rdf:about="http://example.org/onto/prop/google_cloud_run_v2_job_instances">
    <rdfs:label>instances</rdfs:label>
    <rdfs:comment>The Cloud SQL instance connection names, as can be found in https://console.cloud.google.com/sql/instances. Visit https://cloud.google.com/sql/docs/mysql/connect-run for more information on how to connect Cloud SQL and Cloud Run. Format: {project}:{location}:{instance}</rdfs:comment>
    <rdfs:domain rdf:resource="http://example.org/onto/class/google_cloud_run_v2_job"/>
    <rdfs:range rdf:resource="http://www.w3.org/2001/XMLSchema#string"/>
  </owl:DatatypeProperty>
  <owl:DatatypeProperty rdf:about="http://example.org/onto/prop/google_cloud_run_v2_job_medium">
    <rdfs:label>medium</rdfs:label>
    <rdfs:comment>The different types of medium supported for EmptyDir. Default value: "MEMORY" Possible values: ["MEMORY"]</rdfs:comment>
    <rdfs:domain rdf:resource="http://example.org/onto/class/google_cloud_run_v2_job"/>
    <rdfs:range rdf:resource="http://www.w3.org/2001/XMLSchema#string"/>
  </owl:DatatypeProperty>
  <owl:DatatypeProperty rdf:about="http://example.org/onto/prop/google_cloud_run_v2_job_size_limit">
    <rdfs:label>size_limit</rdfs:label>
    <rdfs:comment>Limit on the storage usable by this EmptyDir volume. The size limit is also applicable for memory medium. The maximum usage on memory medium EmptyDir would be the minimum value between the SizeLimit specified here and the sum of memory limits of all containers in a pod. This field's values are of the 'Quantity' k8s type: https://kubernetes.io/docs/reference/kubernetes-api/common-definitions/quantity/. The default is nil which means that the limit is undefined. More info: https://kubernetes.io/docs/concepts/storage/volumes/#emptydir.</rdfs:comment>
    <rdfs:domain rdf:resource="http://example.org/onto/class/google_cloud_run_v2_job"/>
    <rdfs:range rdf:resource="http://www.w3.org/2001/XMLSchema#string"/>
  </owl:DatatypeProperty>
  <owl:DatatypeProperty rdf:about="http://example.org/onto/prop/google_cloud_run_v2_job_bucket">
    <rdfs:label>bucket</rdfs:label>
    <rdfs:comment>Name of the cloud storage bucket to back the volume. The resource service account must have permission to access the bucket.</rdfs:comment>
    <rdfs:domain rdf:resource="http://example.org/onto/class/google_cloud_run_v2_job"/>
    <rdfs:range rdf:resource="http://www.w3.org/2001/XMLSchema#string"/>
  </owl:DatatypeProperty>
  <owl:DatatypeProperty rdf:about="http://example.org/onto/prop/google_cloud_run_v2_job_mount_options">
    <rdfs:label>mount_options</rdfs:label>
    <rdfs:comment>A list of flags to pass to the gcsfuse command for configuring this volume.
Flags should be passed without leading dashes.</rdfs:comment>
    <rdfs:domain rdf:resource="http://example.org/onto/class/google_cloud_run_v2_job"/>
    <rdfs:range rdf:resource="http://www.w3.org/2001/XMLSchema#string"/>
  </owl:DatatypeProperty>
  <owl:DatatypeProperty rdf:about="http://example.org/onto/prop/google_cloud_run_v2_job_read_only">
    <rdfs:label>read_only</rdfs:label>
    <rdfs:comment>If true, mount this volume as read-only in all mounts. If false, mount this volume as read-write.</rdfs:comment>
    <rdfs:domain rdf:resource="http://example.org/onto/class/google_cloud_run_v2_job"/>
    <rdfs:range rdf:resource="http://www.w3.org/2001/XMLSchema#string"/>
  </owl:DatatypeProperty>
  <owl:DatatypeProperty rdf:about="http://example.org/onto/prop/google_cloud_run_v2_job_path">
    <rdfs:label>path</rdfs:label>
    <rdfs:comment>Path that is exported by the NFS server.</rdfs:comment>
    <rdfs:domain rdf:resource="http://example.org/onto/class/google_cloud_run_v2_job"/>
    <rdfs:range rdf:resource="http://www.w3.org/2001/XMLSchema#string"/>
  </owl:DatatypeProperty>
  <owl:DatatypeProperty rdf:about="http://example.org/onto/prop/google_cloud_run_v2_job_read_only">
    <rdfs:label>read_only</rdfs:label>
    <rdfs:comment>If true, mount this volume as read-only in all mounts.</rdfs:comment>
    <rdfs:domain rdf:resource="http://example.org/onto/class/google_cloud_run_v2_job"/>
    <rdfs:range rdf:resource="http://www.w3.org/2001/XMLSchema#string"/>
  </owl:DatatypeProperty>
  <owl:DatatypeProperty rdf:about="http://example.org/onto/prop/google_cloud_run_v2_job_server">
    <rdfs:label>server</rdfs:label>
    <rdfs:comment>Hostname or IP address of the NFS server.</rdfs:comment>
    <rdfs:domain rdf:resource="http://example.org/onto/class/google_cloud_run_v2_job"/>
    <rdfs:range rdf:resource="http://www.w3.org/2001/XMLSchema#string"/>
  </owl:DatatypeProperty>
  <owl:DatatypeProperty rdf:about="http://example.org/onto/prop/google_cloud_run_v2_job_default_mode">
    <rdfs:label>default_mode</rdfs:label>
    <rdfs:comment>Integer representation of mode bits to use on created files by default. Must be a value between 0000 and 0777 (octal), defaulting to 0444. Directories within the path are not affected by this setting.</rdfs:comment>
    <rdfs:domain rdf:resource="http://example.org/onto/class/google_cloud_run_v2_job"/>
    <rdfs:range rdf:resource="http://www.w3.org/2001/XMLSchema#string"/>
  </owl:DatatypeProperty>
  <owl:DatatypeProperty rdf:about="http://example.org/onto/prop/google_cloud_run_v2_job_secret">
    <rdfs:label>secret</rdfs:label>
    <rdfs:comment>The name of the secret in Cloud Secret Manager. Format: {secret} if the secret is in the same project. projects/{project}/secrets/{secret} if the secret is in a different project.</rdfs:comment>
    <rdfs:domain rdf:resource="http://example.org/onto/class/google_cloud_run_v2_job"/>
    <rdfs:range rdf:resource="http://www.w3.org/2001/XMLSchema#string"/>
  </owl:DatatypeProperty>
  <owl:DatatypeProperty rdf:about="http://example.org/onto/prop/google_cloud_run_v2_job_mode">
    <rdfs:label>mode</rdfs:label>
    <rdfs:comment>Integer octal mode bits to use on this file, must be a value between 01 and 0777 (octal). If 0 or not set, the Volume's default mode will be used.</rdfs:comment>
    <rdfs:domain rdf:resource="http://example.org/onto/class/google_cloud_run_v2_job"/>
    <rdfs:range rdf:resource="http://www.w3.org/2001/XMLSchema#string"/>
  </owl:DatatypeProperty>
  <owl:DatatypeProperty rdf:about="http://example.org/onto/prop/google_cloud_run_v2_job_path">
    <rdfs:label>path</rdfs:label>
    <rdfs:comment>The relative path of the secret in the container.</rdfs:comment>
    <rdfs:domain rdf:resource="http://example.org/onto/class/google_cloud_run_v2_job"/>
    <rdfs:range rdf:resource="http://www.w3.org/2001/XMLSchema#string"/>
  </owl:DatatypeProperty>
  <owl:DatatypeProperty rdf:about="http://example.org/onto/prop/google_cloud_run_v2_job_version">
    <rdfs:label>version</rdfs:label>
    <rdfs:comment>The Cloud Secret Manager secret version. Can be 'latest' for the latest value or an integer for a specific version</rdfs:comment>
    <rdfs:domain rdf:resource="http://example.org/onto/class/google_cloud_run_v2_job"/>
    <rdfs:range rdf:resource="http://www.w3.org/2001/XMLSchema#string"/>
  </owl:DatatypeProperty>
  <owl:DatatypeProperty rdf:about="http://example.org/onto/prop/google_cloud_run_v2_job_connector">
    <rdfs:label>connector</rdfs:label>
    <rdfs:comment>VPC Access connector name. Format: projects/{project}/locations/{location}/connectors/{connector}, where {project} can be project id or number.</rdfs:comment>
    <rdfs:domain rdf:resource="http://example.org/onto/class/google_cloud_run_v2_job"/>
    <rdfs:range rdf:resource="http://www.w3.org/2001/XMLSchema#string"/>
  </owl:DatatypeProperty>
  <owl:DatatypeProperty rdf:about="http://example.org/onto/prop/google_cloud_run_v2_job_egress">
    <rdfs:label>egress</rdfs:label>
    <rdfs:comment>Traffic VPC egress settings. Possible values: ["ALL_TRAFFIC", "PRIVATE_RANGES_ONLY"]</rdfs:comment>
    <rdfs:domain rdf:resource="http://example.org/onto/class/google_cloud_run_v2_job"/>
    <rdfs:range rdf:resource="http://www.w3.org/2001/XMLSchema#string"/>
  </owl:DatatypeProperty>
  <owl:DatatypeProperty rdf:about="http://example.org/onto/prop/google_cloud_run_v2_job_network">
    <rdfs:label>network</rdfs:label>
    <rdfs:comment>The VPC network that the Cloud Run resource will be able to send traffic to. At least one of network or subnetwork must be specified. If both
network and subnetwork are specified, the given VPC subnetwork must belong to the given VPC network. If network is not specified, it will be
looked up from the subnetwork.</rdfs:comment>
    <rdfs:domain rdf:resource="http://example.org/onto/class/google_cloud_run_v2_job"/>
    <rdfs:range rdf:resource="http://www.w3.org/2001/XMLSchema#string"/>
  </owl:DatatypeProperty>
  <owl:DatatypeProperty rdf:about="http://example.org/onto/prop/google_cloud_run_v2_job_subnetwork">
    <rdfs:label>subnetwork</rdfs:label>
    <rdfs:comment>The VPC subnetwork that the Cloud Run resource will get IPs from. At least one of network or subnetwork must be specified. If both
network and subnetwork are specified, the given VPC subnetwork must belong to the given VPC network. If subnetwork is not specified, the
subnetwork with the same name with the network will be used.</rdfs:comment>
    <rdfs:domain rdf:resource="http://example.org/onto/class/google_cloud_run_v2_job"/>
    <rdfs:range rdf:resource="http://www.w3.org/2001/XMLSchema#string"/>
  </owl:DatatypeProperty>
  <owl:DatatypeProperty rdf:about="http://example.org/onto/prop/google_cloud_run_v2_job_tags">
    <rdfs:label>tags</rdfs:label>
    <rdfs:comment>Network tags applied to this Cloud Run job.</rdfs:comment>
    <rdfs:domain rdf:resource="http://example.org/onto/class/google_cloud_run_v2_job"/>
    <rdfs:range rdf:resource="http://www.w3.org/2001/XMLSchema#string"/>
  </owl:DatatypeProperty>
  <owl:DatatypeProperty rdf:about="http://example.org/onto/prop/google_cloud_run_v2_job_create">
    <rdfs:label>create</rdfs:label>
    <rdfs:domain rdf:resource="http://example.org/onto/class/google_cloud_run_v2_job"/>
    <rdfs:range rdf:resource="http://www.w3.org/2001/XMLSchema#string"/>
  </owl:DatatypeProperty>
  <owl:DatatypeProperty rdf:about="http://example.org/onto/prop/google_cloud_run_v2_job_delete">
    <rdfs:label>delete</rdfs:label>
    <rdfs:domain rdf:resource="http://example.org/onto/class/google_cloud_run_v2_job"/>
    <rdfs:range rdf:resource="http://www.w3.org/2001/XMLSchema#string"/>
  </owl:DatatypeProperty>
  <owl:DatatypeProperty rdf:about="http://example.org/onto/prop/google_cloud_run_v2_job_update">
    <rdfs:label>update</rdfs:label>
    <rdfs:domain rdf:resource="http://example.org/onto/class/google_cloud_run_v2_job"/>
    <rdfs:range rdf:resource="http://www.w3.org/2001/XMLSchema#string"/>
  </owl:DatatypeProperty>
</rdf:RDF>
