<?xml version="1.0" encoding="UTF-8"?>
<rdf:RDF
  xmlns:rdf="http://www.w3.org/1999/02/22-rdf-syntax-ns#"
  xmlns:rdfs="http://www.w3.org/2000/01/rdf-schema#"
  xmlns:owl="http://www.w3.org/2002/07/owl#"
  xmlns:xsd="http://www.w3.org/2001/XMLSchema#"
  xml:base="http://example.org/onto/">
  <owl:Class rdf:about="http://example.org/onto/class/google_model_armor_floorsetting">
    <rdfs:label>google_model_armor_floorsetting</rdfs:label>
    <rdfs:comment>#
#     ***     AUTO GENERATED CODE    ***    Type: MMv1     ***
#
# ----------------------------------------------------------------------------
#
#     This code is generated by Magic Modules using the following:
#
#     Configuration: https:#github.com/GoogleCloudPlatform/magic-modules/tree/main/mmv1/products/modelarmorglobal/Floorsetting.yaml
#     Template:      https:#github.com/GoogleCloudPlatform/magic-modules/tree/main/mmv1/templates/terraform/resource.html.markdown.tmpl
#
#     DO NOT EDIT this file directly. Any changes made to this file will be
#     overwritten during the next generation cycle.
#
# ----------------------------------------------------------------------------
subcategory: "Model Armor"
description: |-
  Model Armor floor settings define rules that dictate minimum requirements for all Model Armor templates created at a specific point in the Google Cloud resource hierarchy (that is, at an organization, folder, or project level).
---</rdfs:comment>
  </owl:Class>
  <owl:DatatypeProperty rdf:about="http://example.org/onto/prop/google_model_armor_floorsetting_create_time">
    <rdfs:label>create_time</rdfs:label>
    <rdfs:comment>[Output only] Create timestamp</rdfs:comment>
    <rdfs:domain rdf:resource="http://example.org/onto/class/google_model_armor_floorsetting"/>
    <rdfs:range rdf:resource="http://www.w3.org/2001/XMLSchema#string"/>
  </owl:DatatypeProperty>
  <owl:DatatypeProperty rdf:about="http://example.org/onto/prop/google_model_armor_floorsetting_enable_floor_setting_enforcement">
    <rdfs:label>enable_floor_setting_enforcement</rdfs:label>
    <rdfs:comment>Floor Settings enforcement status.</rdfs:comment>
    <rdfs:domain rdf:resource="http://example.org/onto/class/google_model_armor_floorsetting"/>
    <rdfs:range rdf:resource="http://www.w3.org/2001/XMLSchema#string"/>
  </owl:DatatypeProperty>
  <owl:DatatypeProperty rdf:about="http://example.org/onto/prop/google_model_armor_floorsetting_id">
    <rdfs:label>id</rdfs:label>
    <rdfs:domain rdf:resource="http://example.org/onto/class/google_model_armor_floorsetting"/>
    <rdfs:range rdf:resource="http://www.w3.org/2001/XMLSchema#string"/>
  </owl:DatatypeProperty>
  <owl:DatatypeProperty rdf:about="http://example.org/onto/prop/google_model_armor_floorsetting_integrated_services">
    <rdfs:label>integrated_services</rdfs:label>
    <rdfs:comment>List of integrated services for which the floor setting is applicable.</rdfs:comment>
    <rdfs:domain rdf:resource="http://example.org/onto/class/google_model_armor_floorsetting"/>
    <rdfs:range rdf:resource="http://www.w3.org/2001/XMLSchema#string"/>
  </owl:DatatypeProperty>
  <owl:DatatypeProperty rdf:about="http://example.org/onto/prop/google_model_armor_floorsetting_location">
    <rdfs:label>location</rdfs:label>
    <rdfs:comment>Resource ID segment making up resource 'name'. It identifies the resource within its parent collection as described in https://google.aip.dev/122.</rdfs:comment>
    <rdfs:domain rdf:resource="http://example.org/onto/class/google_model_armor_floorsetting"/>
    <rdfs:range rdf:resource="http://www.w3.org/2001/XMLSchema#string"/>
  </owl:DatatypeProperty>
  <owl:DatatypeProperty rdf:about="http://example.org/onto/prop/google_model_armor_floorsetting_name">
    <rdfs:label>name</rdfs:label>
    <rdfs:comment>Identifier. The resource name.</rdfs:comment>
    <rdfs:domain rdf:resource="http://example.org/onto/class/google_model_armor_floorsetting"/>
    <rdfs:range rdf:resource="http://www.w3.org/2001/XMLSchema#string"/>
  </owl:DatatypeProperty>
  <owl:DatatypeProperty rdf:about="http://example.org/onto/prop/google_model_armor_floorsetting_parent">
    <rdfs:label>parent</rdfs:label>
    <rdfs:comment>Will be any one of these:

* 'projects/{project}'
* 'folders/{folder}'
* 'organizations/{organizationId}'</rdfs:comment>
    <rdfs:domain rdf:resource="http://example.org/onto/class/google_model_armor_floorsetting"/>
    <rdfs:range rdf:resource="http://www.w3.org/2001/XMLSchema#string"/>
  </owl:DatatypeProperty>
  <owl:DatatypeProperty rdf:about="http://example.org/onto/prop/google_model_armor_floorsetting_update_time">
    <rdfs:label>update_time</rdfs:label>
    <rdfs:comment>[Output only] Update timestamp</rdfs:comment>
    <rdfs:domain rdf:resource="http://example.org/onto/class/google_model_armor_floorsetting"/>
    <rdfs:range rdf:resource="http://www.w3.org/2001/XMLSchema#string"/>
  </owl:DatatypeProperty>
  <owl:DatatypeProperty rdf:about="http://example.org/onto/prop/google_model_armor_floorsetting_enable_cloud_logging">
    <rdfs:label>enable_cloud_logging</rdfs:label>
    <rdfs:comment>If true, log Model Armor filter results to Cloud Logging.</rdfs:comment>
    <rdfs:domain rdf:resource="http://example.org/onto/class/google_model_armor_floorsetting"/>
    <rdfs:range rdf:resource="http://www.w3.org/2001/XMLSchema#string"/>
  </owl:DatatypeProperty>
  <owl:DatatypeProperty rdf:about="http://example.org/onto/prop/google_model_armor_floorsetting_inspect_and_block">
    <rdfs:label>inspect_and_block</rdfs:label>
    <rdfs:comment>If true, Model Armor filters will be run in inspect and block mode.
Requests that trip Model Armor filters will be blocked.</rdfs:comment>
    <rdfs:domain rdf:resource="http://example.org/onto/class/google_model_armor_floorsetting"/>
    <rdfs:range rdf:resource="http://www.w3.org/2001/XMLSchema#string"/>
  </owl:DatatypeProperty>
  <owl:DatatypeProperty rdf:about="http://example.org/onto/prop/google_model_armor_floorsetting_inspect_only">
    <rdfs:label>inspect_only</rdfs:label>
    <rdfs:comment>If true, Model Armor filters will be run in inspect only mode. No action
will be taken on the request.</rdfs:comment>
    <rdfs:domain rdf:resource="http://example.org/onto/class/google_model_armor_floorsetting"/>
    <rdfs:range rdf:resource="http://www.w3.org/2001/XMLSchema#string"/>
  </owl:DatatypeProperty>
  <owl:DatatypeProperty rdf:about="http://example.org/onto/prop/google_model_armor_floorsetting_filter_enforcement">
    <rdfs:label>filter_enforcement</rdfs:label>
    <rdfs:comment>Tells whether the Malicious URI filter is enabled or disabled.
Possible values:
ENABLED
DISABLED</rdfs:comment>
    <rdfs:domain rdf:resource="http://example.org/onto/class/google_model_armor_floorsetting"/>
    <rdfs:range rdf:resource="http://www.w3.org/2001/XMLSchema#string"/>
  </owl:DatatypeProperty>
  <owl:DatatypeProperty rdf:about="http://example.org/onto/prop/google_model_armor_floorsetting_confidence_level">
    <rdfs:label>confidence_level</rdfs:label>
    <rdfs:comment>Possible values:
LOW_AND_ABOVE
MEDIUM_AND_ABOVE
HIGH</rdfs:comment>
    <rdfs:domain rdf:resource="http://example.org/onto/class/google_model_armor_floorsetting"/>
    <rdfs:range rdf:resource="http://www.w3.org/2001/XMLSchema#string"/>
  </owl:DatatypeProperty>
  <owl:DatatypeProperty rdf:about="http://example.org/onto/prop/google_model_armor_floorsetting_filter_enforcement">
    <rdfs:label>filter_enforcement</rdfs:label>
    <rdfs:comment>Tells whether Prompt injection and Jailbreak filter is enabled or
disabled.
Possible values:
ENABLED
DISABLED</rdfs:comment>
    <rdfs:domain rdf:resource="http://example.org/onto/class/google_model_armor_floorsetting"/>
    <rdfs:range rdf:resource="http://www.w3.org/2001/XMLSchema#string"/>
  </owl:DatatypeProperty>
  <owl:DatatypeProperty rdf:about="http://example.org/onto/prop/google_model_armor_floorsetting_confidence_level">
    <rdfs:label>confidence_level</rdfs:label>
    <rdfs:comment>Possible values:
LOW_AND_ABOVE
MEDIUM_AND_ABOVE
HIGH</rdfs:comment>
    <rdfs:domain rdf:resource="http://example.org/onto/class/google_model_armor_floorsetting"/>
    <rdfs:range rdf:resource="http://www.w3.org/2001/XMLSchema#string"/>
  </owl:DatatypeProperty>
  <owl:DatatypeProperty rdf:about="http://example.org/onto/prop/google_model_armor_floorsetting_filter_type">
    <rdfs:label>filter_type</rdfs:label>
    <rdfs:comment>Possible values:
SEXUALLY_EXPLICIT
HATE_SPEECH
HARASSMENT
DANGEROUS</rdfs:comment>
    <rdfs:domain rdf:resource="http://example.org/onto/class/google_model_armor_floorsetting"/>
    <rdfs:range rdf:resource="http://www.w3.org/2001/XMLSchema#string"/>
  </owl:DatatypeProperty>
  <owl:DatatypeProperty rdf:about="http://example.org/onto/prop/google_model_armor_floorsetting_deidentify_template">
    <rdfs:label>deidentify_template</rdfs:label>
    <rdfs:comment>Optional Sensitive Data Protection Deidentify template resource name.

If provided then DeidentifyContent action is performed during Sanitization
using this template and inspect template. The De-identified data will
be returned in SdpDeidentifyResult.
Note that all info-types present in the deidentify template must be present
in inspect template.

e.g.
'projects/{project}/locations/{location}/deidentifyTemplates/{deidentify_template}'</rdfs:comment>
    <rdfs:domain rdf:resource="http://example.org/onto/class/google_model_armor_floorsetting"/>
    <rdfs:range rdf:resource="http://www.w3.org/2001/XMLSchema#string"/>
  </owl:DatatypeProperty>
  <owl:DatatypeProperty rdf:about="http://example.org/onto/prop/google_model_armor_floorsetting_inspect_template">
    <rdfs:label>inspect_template</rdfs:label>
    <rdfs:comment>Sensitive Data Protection inspect template resource name

If only inspect template is provided (de-identify template not provided),
then Sensitive Data Protection InspectContent action is performed during
Sanitization. All Sensitive Data Protection findings identified during
inspection will be returned as SdpFinding in SdpInsepctionResult.

e.g:-
'projects/{project}/locations/{location}/inspectTemplates/{inspect_template}'</rdfs:comment>
    <rdfs:domain rdf:resource="http://example.org/onto/class/google_model_armor_floorsetting"/>
    <rdfs:range rdf:resource="http://www.w3.org/2001/XMLSchema#string"/>
  </owl:DatatypeProperty>
  <owl:DatatypeProperty rdf:about="http://example.org/onto/prop/google_model_armor_floorsetting_filter_enforcement">
    <rdfs:label>filter_enforcement</rdfs:label>
    <rdfs:comment>Tells whether the Sensitive Data Protection basic config is enabled or
disabled.
Possible values:
ENABLED
DISABLED</rdfs:comment>
    <rdfs:domain rdf:resource="http://example.org/onto/class/google_model_armor_floorsetting"/>
    <rdfs:range rdf:resource="http://www.w3.org/2001/XMLSchema#string"/>
  </owl:DatatypeProperty>
  <owl:DatatypeProperty rdf:about="http://example.org/onto/prop/google_model_armor_floorsetting_enable_multi_language_detection">
    <rdfs:label>enable_multi_language_detection</rdfs:label>
    <rdfs:comment>If true, multi language detection will be enabled.</rdfs:comment>
    <rdfs:domain rdf:resource="http://example.org/onto/class/google_model_armor_floorsetting"/>
    <rdfs:range rdf:resource="http://www.w3.org/2001/XMLSchema#string"/>
  </owl:DatatypeProperty>
  <owl:DatatypeProperty rdf:about="http://example.org/onto/prop/google_model_armor_floorsetting_create">
    <rdfs:label>create</rdfs:label>
    <rdfs:domain rdf:resource="http://example.org/onto/class/google_model_armor_floorsetting"/>
    <rdfs:range rdf:resource="http://www.w3.org/2001/XMLSchema#string"/>
  </owl:DatatypeProperty>
  <owl:DatatypeProperty rdf:about="http://example.org/onto/prop/google_model_armor_floorsetting_delete">
    <rdfs:label>delete</rdfs:label>
    <rdfs:domain rdf:resource="http://example.org/onto/class/google_model_armor_floorsetting"/>
    <rdfs:range rdf:resource="http://www.w3.org/2001/XMLSchema#string"/>
  </owl:DatatypeProperty>
  <owl:DatatypeProperty rdf:about="http://example.org/onto/prop/google_model_armor_floorsetting_update">
    <rdfs:label>update</rdfs:label>
    <rdfs:domain rdf:resource="http://example.org/onto/class/google_model_armor_floorsetting"/>
    <rdfs:range rdf:resource="http://www.w3.org/2001/XMLSchema#string"/>
  </owl:DatatypeProperty>
</rdf:RDF>
