<?xml version="1.0" encoding="UTF-8"?>
<rdf:RDF
  xmlns:rdf="http://www.w3.org/1999/02/22-rdf-syntax-ns#"
  xmlns:rdfs="http://www.w3.org/2000/01/rdf-schema#"
  xmlns:owl="http://www.w3.org/2002/07/owl#"
  xmlns:xsd="http://www.w3.org/2001/XMLSchema#"
  xml:base="http://example.org/onto/">
  <owl:Class rdf:about="http://example.org/onto/class/google_dialogflow_conversation_profile">
    <rdfs:label>google_dialogflow_conversation_profile</rdfs:label>
    <rdfs:comment>#
#     ***     AUTO GENERATED CODE    ***    Type: MMv1     ***
#
# ----------------------------------------------------------------------------
#
#     This code is generated by Magic Modules using the following:
#
#     Configuration: https:#github.com/GoogleCloudPlatform/magic-modules/tree/main/mmv1/products/dialogflow/ConversationProfile.yaml
#     Template:      https:#github.com/GoogleCloudPlatform/magic-modules/tree/main/mmv1/templates/terraform/resource.html.markdown.tmpl
#
#     DO NOT EDIT this file directly. Any changes made to this file will be
#     overwritten during the next generation cycle.
#
# ----------------------------------------------------------------------------
subcategory: "Dialogflow"
description: |-
  A conversation profile configures a set of parameters that control the suggestions made to an agent.
---</rdfs:comment>
  </owl:Class>
  <owl:DatatypeProperty rdf:about="http://example.org/onto/prop/google_dialogflow_conversation_profile_display_name">
    <rdfs:label>display_name</rdfs:label>
    <rdfs:comment>Required. Human readable name for this profile. Max length 1024 bytes.</rdfs:comment>
    <rdfs:domain rdf:resource="http://example.org/onto/class/google_dialogflow_conversation_profile"/>
    <rdfs:range rdf:resource="http://www.w3.org/2001/XMLSchema#string"/>
  </owl:DatatypeProperty>
  <owl:DatatypeProperty rdf:about="http://example.org/onto/prop/google_dialogflow_conversation_profile_id">
    <rdfs:label>id</rdfs:label>
    <rdfs:domain rdf:resource="http://example.org/onto/class/google_dialogflow_conversation_profile"/>
    <rdfs:range rdf:resource="http://www.w3.org/2001/XMLSchema#string"/>
  </owl:DatatypeProperty>
  <owl:DatatypeProperty rdf:about="http://example.org/onto/prop/google_dialogflow_conversation_profile_language_code">
    <rdfs:label>language_code</rdfs:label>
    <rdfs:comment>Language code for the conversation profile. This should be a BCP-47 language tag.</rdfs:comment>
    <rdfs:domain rdf:resource="http://example.org/onto/class/google_dialogflow_conversation_profile"/>
    <rdfs:range rdf:resource="http://www.w3.org/2001/XMLSchema#string"/>
  </owl:DatatypeProperty>
  <owl:DatatypeProperty rdf:about="http://example.org/onto/prop/google_dialogflow_conversation_profile_location">
    <rdfs:label>location</rdfs:label>
    <rdfs:comment>desc</rdfs:comment>
    <rdfs:domain rdf:resource="http://example.org/onto/class/google_dialogflow_conversation_profile"/>
    <rdfs:range rdf:resource="http://www.w3.org/2001/XMLSchema#string"/>
  </owl:DatatypeProperty>
  <owl:DatatypeProperty rdf:about="http://example.org/onto/prop/google_dialogflow_conversation_profile_name">
    <rdfs:label>name</rdfs:label>
    <rdfs:comment>name</rdfs:comment>
    <rdfs:domain rdf:resource="http://example.org/onto/class/google_dialogflow_conversation_profile"/>
    <rdfs:range rdf:resource="http://www.w3.org/2001/XMLSchema#string"/>
  </owl:DatatypeProperty>
  <owl:DatatypeProperty rdf:about="http://example.org/onto/prop/google_dialogflow_conversation_profile_project">
    <rdfs:label>project</rdfs:label>
    <rdfs:domain rdf:resource="http://example.org/onto/class/google_dialogflow_conversation_profile"/>
    <rdfs:range rdf:resource="http://www.w3.org/2001/XMLSchema#string"/>
  </owl:DatatypeProperty>
  <owl:DatatypeProperty rdf:about="http://example.org/onto/prop/google_dialogflow_conversation_profile_security_settings">
    <rdfs:label>security_settings</rdfs:label>
    <rdfs:comment>Name of the CX SecuritySettings reference for the agent.</rdfs:comment>
    <rdfs:domain rdf:resource="http://example.org/onto/class/google_dialogflow_conversation_profile"/>
    <rdfs:range rdf:resource="http://www.w3.org/2001/XMLSchema#string"/>
  </owl:DatatypeProperty>
  <owl:DatatypeProperty rdf:about="http://example.org/onto/prop/google_dialogflow_conversation_profile_time_zone">
    <rdfs:label>time_zone</rdfs:label>
    <rdfs:comment>The time zone of this conversational profile.</rdfs:comment>
    <rdfs:domain rdf:resource="http://example.org/onto/class/google_dialogflow_conversation_profile"/>
    <rdfs:range rdf:resource="http://www.w3.org/2001/XMLSchema#string"/>
  </owl:DatatypeProperty>
  <owl:DatatypeProperty rdf:about="http://example.org/onto/prop/google_dialogflow_conversation_profile_agent">
    <rdfs:label>agent</rdfs:label>
    <rdfs:comment>ID of the Dialogflow agent environment to use.
Expects the format "projects/<Project ID>/locations/<Location ID>/agent/environments/<EnvironmentID>"</rdfs:comment>
    <rdfs:domain rdf:resource="http://example.org/onto/class/google_dialogflow_conversation_profile"/>
    <rdfs:range rdf:resource="http://www.w3.org/2001/XMLSchema#string"/>
  </owl:DatatypeProperty>
  <owl:DatatypeProperty rdf:about="http://example.org/onto/prop/google_dialogflow_conversation_profile_session_ttl">
    <rdfs:label>session_ttl</rdfs:label>
    <rdfs:comment>Configure lifetime of the Dialogflow session.</rdfs:comment>
    <rdfs:domain rdf:resource="http://example.org/onto/class/google_dialogflow_conversation_profile"/>
    <rdfs:range rdf:resource="http://www.w3.org/2001/XMLSchema#string"/>
  </owl:DatatypeProperty>
  <owl:DatatypeProperty rdf:about="http://example.org/onto/prop/google_dialogflow_conversation_profile_disable_high_latency_features_sync_delivery">
    <rdfs:label>disable_high_latency_features_sync_delivery</rdfs:label>
    <rdfs:comment>When disableHighLatencyFeaturesSyncDelivery is true and using the AnalyzeContent API, we will not deliver the responses from high latency features in the API response. The humanAgentAssistantConfig.notification_config must be configured and enableEventBasedSuggestion must be set to true to receive the responses from high latency features in Pub/Sub. High latency feature(s): KNOWLEDGE_ASSIST</rdfs:comment>
    <rdfs:domain rdf:resource="http://example.org/onto/class/google_dialogflow_conversation_profile"/>
    <rdfs:range rdf:resource="http://www.w3.org/2001/XMLSchema#string"/>
  </owl:DatatypeProperty>
  <owl:DatatypeProperty rdf:about="http://example.org/onto/prop/google_dialogflow_conversation_profile_generators">
    <rdfs:label>generators</rdfs:label>
    <rdfs:comment>List of various generator resource names used in the conversation profile.</rdfs:comment>
    <rdfs:domain rdf:resource="http://example.org/onto/class/google_dialogflow_conversation_profile"/>
    <rdfs:range rdf:resource="http://www.w3.org/2001/XMLSchema#string"/>
  </owl:DatatypeProperty>
  <owl:DatatypeProperty rdf:about="http://example.org/onto/prop/google_dialogflow_conversation_profile_group_suggestion_responses">
    <rdfs:label>group_suggestion_responses</rdfs:label>
    <rdfs:comment>If groupSuggestionResponses is false, and there are multiple featureConfigs in event based suggestion or StreamingAnalyzeContent, we will try to deliver suggestions to customers as soon as we get new suggestion. Different type of suggestions based on the same context will be in separate Pub/Sub event or StreamingAnalyzeContentResponse.

If groupSuggestionResponses set to true. All the suggestions to the same participant based on the same context will be grouped into a single Pub/Sub event or StreamingAnalyzeContentResponse.</rdfs:comment>
    <rdfs:domain rdf:resource="http://example.org/onto/class/google_dialogflow_conversation_profile"/>
    <rdfs:range rdf:resource="http://www.w3.org/2001/XMLSchema#string"/>
  </owl:DatatypeProperty>
  <owl:DatatypeProperty rdf:about="http://example.org/onto/prop/google_dialogflow_conversation_profile_disable_agent_query_logging">
    <rdfs:label>disable_agent_query_logging</rdfs:label>
    <rdfs:comment>Disable the logging of search queries sent by human agents. It can prevent those queries from being stored at answer records.
This feature is only supported for types: KNOWLEDGE_SEARCH.</rdfs:comment>
    <rdfs:domain rdf:resource="http://example.org/onto/class/google_dialogflow_conversation_profile"/>
    <rdfs:range rdf:resource="http://www.w3.org/2001/XMLSchema#string"/>
  </owl:DatatypeProperty>
  <owl:DatatypeProperty rdf:about="http://example.org/onto/prop/google_dialogflow_conversation_profile_enable_conversation_augmented_query">
    <rdfs:label>enable_conversation_augmented_query</rdfs:label>
    <rdfs:comment>Enable including conversation context during query answer generation.
This feature is only supported for types: KNOWLEDGE_SEARCH.</rdfs:comment>
    <rdfs:domain rdf:resource="http://example.org/onto/class/google_dialogflow_conversation_profile"/>
    <rdfs:range rdf:resource="http://www.w3.org/2001/XMLSchema#string"/>
  </owl:DatatypeProperty>
  <owl:DatatypeProperty rdf:about="http://example.org/onto/prop/google_dialogflow_conversation_profile_enable_event_based_suggestion">
    <rdfs:label>enable_event_based_suggestion</rdfs:label>
    <rdfs:comment>Automatically iterates all participants and tries to compile suggestions.
This feature is only supported for types: ARTICLE_SUGGESTION, FAQ, DIALOGFLOW_ASSIST, KNOWLEDGE_ASSIST.</rdfs:comment>
    <rdfs:domain rdf:resource="http://example.org/onto/class/google_dialogflow_conversation_profile"/>
    <rdfs:range rdf:resource="http://www.w3.org/2001/XMLSchema#string"/>
  </owl:DatatypeProperty>
  <owl:DatatypeProperty rdf:about="http://example.org/onto/prop/google_dialogflow_conversation_profile_enable_query_suggestion_only">
    <rdfs:label>enable_query_suggestion_only</rdfs:label>
    <rdfs:comment>Enable query suggestion only.
This feature is only supported for types: KNOWLEDGE_ASSIST</rdfs:comment>
    <rdfs:domain rdf:resource="http://example.org/onto/class/google_dialogflow_conversation_profile"/>
    <rdfs:range rdf:resource="http://www.w3.org/2001/XMLSchema#string"/>
  </owl:DatatypeProperty>
  <owl:DatatypeProperty rdf:about="http://example.org/onto/prop/google_dialogflow_conversation_profile_enable_query_suggestion_when_no_answer">
    <rdfs:label>enable_query_suggestion_when_no_answer</rdfs:label>
    <rdfs:comment>Enable query suggestion even if we can't find its answer. By default, queries are suggested only if we find its answer.
This feature is only supported for types: KNOWLEDGE_ASSIST.</rdfs:comment>
    <rdfs:domain rdf:resource="http://example.org/onto/class/google_dialogflow_conversation_profile"/>
    <rdfs:range rdf:resource="http://www.w3.org/2001/XMLSchema#string"/>
  </owl:DatatypeProperty>
  <owl:DatatypeProperty rdf:about="http://example.org/onto/prop/google_dialogflow_conversation_profile_baseline_model_version">
    <rdfs:label>baseline_model_version</rdfs:label>
    <rdfs:comment>Version of current baseline model. It will be ignored if model is set. Valid versions are: Article Suggestion baseline model: - 0.9 - 1.0 (default) Summarization baseline model: - 1.0</rdfs:comment>
    <rdfs:domain rdf:resource="http://example.org/onto/class/google_dialogflow_conversation_profile"/>
    <rdfs:range rdf:resource="http://www.w3.org/2001/XMLSchema#string"/>
  </owl:DatatypeProperty>
  <owl:DatatypeProperty rdf:about="http://example.org/onto/prop/google_dialogflow_conversation_profile_model">
    <rdfs:label>model</rdfs:label>
    <rdfs:comment>Conversation model resource name. Format: projects/<Project ID>/conversationModels/<Model ID>.</rdfs:comment>
    <rdfs:domain rdf:resource="http://example.org/onto/class/google_dialogflow_conversation_profile"/>
    <rdfs:range rdf:resource="http://www.w3.org/2001/XMLSchema#string"/>
  </owl:DatatypeProperty>
  <owl:DatatypeProperty rdf:about="http://example.org/onto/prop/google_dialogflow_conversation_profile_recent_sentences_count">
    <rdfs:label>recent_sentences_count</rdfs:label>
    <rdfs:comment>Number of recent non-small-talk sentences to use as context for article and FAQ suggestion</rdfs:comment>
    <rdfs:domain rdf:resource="http://example.org/onto/class/google_dialogflow_conversation_profile"/>
    <rdfs:range rdf:resource="http://www.w3.org/2001/XMLSchema#string"/>
  </owl:DatatypeProperty>
  <owl:DatatypeProperty rdf:about="http://example.org/onto/prop/google_dialogflow_conversation_profile_confidence_threshold">
    <rdfs:label>confidence_threshold</rdfs:label>
    <rdfs:comment>Confidence threshold of query result.
This feature is only supported for types: ARTICLE_SUGGESTION, FAQ, SMART_REPLY, SMART_COMPOSE, KNOWLEDGE_SEARCH, KNOWLEDGE_ASSIST, ENTITY_EXTRACTION.</rdfs:comment>
    <rdfs:domain rdf:resource="http://example.org/onto/class/google_dialogflow_conversation_profile"/>
    <rdfs:range rdf:resource="http://www.w3.org/2001/XMLSchema#string"/>
  </owl:DatatypeProperty>
  <owl:DatatypeProperty rdf:about="http://example.org/onto/prop/google_dialogflow_conversation_profile_max_results">
    <rdfs:label>max_results</rdfs:label>
    <rdfs:comment>Maximum number of results to return.</rdfs:comment>
    <rdfs:domain rdf:resource="http://example.org/onto/class/google_dialogflow_conversation_profile"/>
    <rdfs:range rdf:resource="http://www.w3.org/2001/XMLSchema#string"/>
  </owl:DatatypeProperty>
  <owl:DatatypeProperty rdf:about="http://example.org/onto/prop/google_dialogflow_conversation_profile_drop_handoff_messages">
    <rdfs:label>drop_handoff_messages</rdfs:label>
    <rdfs:comment>If set to true, the last message from virtual agent (hand off message) and the message before it (trigger message of hand off) are dropped.</rdfs:comment>
    <rdfs:domain rdf:resource="http://example.org/onto/class/google_dialogflow_conversation_profile"/>
    <rdfs:range rdf:resource="http://www.w3.org/2001/XMLSchema#string"/>
  </owl:DatatypeProperty>
  <owl:DatatypeProperty rdf:about="http://example.org/onto/prop/google_dialogflow_conversation_profile_drop_ivr_messages">
    <rdfs:label>drop_ivr_messages</rdfs:label>
    <rdfs:comment>If set to true, all messages from ivr stage are dropped.</rdfs:comment>
    <rdfs:domain rdf:resource="http://example.org/onto/class/google_dialogflow_conversation_profile"/>
    <rdfs:range rdf:resource="http://www.w3.org/2001/XMLSchema#string"/>
  </owl:DatatypeProperty>
  <owl:DatatypeProperty rdf:about="http://example.org/onto/prop/google_dialogflow_conversation_profile_drop_virtual_agent_messages">
    <rdfs:label>drop_virtual_agent_messages</rdfs:label>
    <rdfs:comment>If set to true, all messages from virtual agent are dropped.</rdfs:comment>
    <rdfs:domain rdf:resource="http://example.org/onto/class/google_dialogflow_conversation_profile"/>
    <rdfs:range rdf:resource="http://www.w3.org/2001/XMLSchema#string"/>
  </owl:DatatypeProperty>
  <owl:DatatypeProperty rdf:about="http://example.org/onto/prop/google_dialogflow_conversation_profile_agent">
    <rdfs:label>agent</rdfs:label>
    <rdfs:comment>he name of a Dialogflow virtual agent used for end user side intent detection and suggestion. Format: projects/<Project ID>/locations/<Location ID>/agent.</rdfs:comment>
    <rdfs:domain rdf:resource="http://example.org/onto/class/google_dialogflow_conversation_profile"/>
    <rdfs:range rdf:resource="http://www.w3.org/2001/XMLSchema#string"/>
  </owl:DatatypeProperty>
  <owl:DatatypeProperty rdf:about="http://example.org/onto/prop/google_dialogflow_conversation_profile_agent">
    <rdfs:label>agent</rdfs:label>
    <rdfs:comment>The name of a dialogflow virtual agent used for intent detection and suggestion triggered by human agent. Format: projects/<Project ID>/locations/<Location ID>/agent.</rdfs:comment>
    <rdfs:domain rdf:resource="http://example.org/onto/class/google_dialogflow_conversation_profile"/>
    <rdfs:range rdf:resource="http://www.w3.org/2001/XMLSchema#string"/>
  </owl:DatatypeProperty>
  <owl:DatatypeProperty rdf:about="http://example.org/onto/prop/google_dialogflow_conversation_profile_documents">
    <rdfs:label>documents</rdfs:label>
    <rdfs:comment>Knowledge documents to query from. Format: projects/<Project ID>/locations/<Location ID>/knowledgeBases/<KnowledgeBase ID>/documents/<Document ID>.</rdfs:comment>
    <rdfs:domain rdf:resource="http://example.org/onto/class/google_dialogflow_conversation_profile"/>
    <rdfs:range rdf:resource="http://www.w3.org/2001/XMLSchema#string"/>
  </owl:DatatypeProperty>
  <owl:DatatypeProperty rdf:about="http://example.org/onto/prop/google_dialogflow_conversation_profile_knowledge_bases">
    <rdfs:label>knowledge_bases</rdfs:label>
    <rdfs:comment>Knowledge bases to query. Format: projects/<Project ID>/locations/<Location ID>/knowledgeBases/<Knowledge Base ID>.</rdfs:comment>
    <rdfs:domain rdf:resource="http://example.org/onto/class/google_dialogflow_conversation_profile"/>
    <rdfs:range rdf:resource="http://www.w3.org/2001/XMLSchema#string"/>
  </owl:DatatypeProperty>
  <owl:DatatypeProperty rdf:about="http://example.org/onto/prop/google_dialogflow_conversation_profile_section_types">
    <rdfs:label>section_types</rdfs:label>
    <rdfs:comment>The selected sections chosen to return when requesting a summary of a conversation
If not provided the default selection will be "{SITUATION, ACTION, RESULT}". Possible values: ["SECTION_TYPE_UNSPECIFIED", "SITUATION", "ACTION", "RESOLUTION", "REASON_FOR_CANCELLATION", "CUSTOMER_SATISFACTION", "ENTITIES"]</rdfs:comment>
    <rdfs:domain rdf:resource="http://example.org/onto/class/google_dialogflow_conversation_profile"/>
    <rdfs:range rdf:resource="http://www.w3.org/2001/XMLSchema#string"/>
  </owl:DatatypeProperty>
  <owl:DatatypeProperty rdf:about="http://example.org/onto/prop/google_dialogflow_conversation_profile_type">
    <rdfs:label>type</rdfs:label>
    <rdfs:comment>Type of Human Agent Assistant API feature to request.</rdfs:comment>
    <rdfs:domain rdf:resource="http://example.org/onto/class/google_dialogflow_conversation_profile"/>
    <rdfs:range rdf:resource="http://www.w3.org/2001/XMLSchema#string"/>
  </owl:DatatypeProperty>
  <owl:DatatypeProperty rdf:about="http://example.org/onto/prop/google_dialogflow_conversation_profile_no_small_talk">
    <rdfs:label>no_small_talk</rdfs:label>
    <rdfs:comment>Do not trigger if last utterance is small talk.</rdfs:comment>
    <rdfs:domain rdf:resource="http://example.org/onto/class/google_dialogflow_conversation_profile"/>
    <rdfs:range rdf:resource="http://www.w3.org/2001/XMLSchema#string"/>
  </owl:DatatypeProperty>
  <owl:DatatypeProperty rdf:about="http://example.org/onto/prop/google_dialogflow_conversation_profile_only_end_user">
    <rdfs:label>only_end_user</rdfs:label>
    <rdfs:comment>Only trigger suggestion if participant role of last utterance is END_USER.</rdfs:comment>
    <rdfs:domain rdf:resource="http://example.org/onto/class/google_dialogflow_conversation_profile"/>
    <rdfs:range rdf:resource="http://www.w3.org/2001/XMLSchema#string"/>
  </owl:DatatypeProperty>
  <owl:DatatypeProperty rdf:about="http://example.org/onto/prop/google_dialogflow_conversation_profile_disable_high_latency_features_sync_delivery">
    <rdfs:label>disable_high_latency_features_sync_delivery</rdfs:label>
    <rdfs:comment>When disableHighLatencyFeaturesSyncDelivery is true and using the AnalyzeContent API, we will not deliver the responses from high latency features in the API response. The humanAgentAssistantConfig.notification_config must be configured and enableEventBasedSuggestion must be set to true to receive the responses from high latency features in Pub/Sub. High latency feature(s): KNOWLEDGE_ASSIST</rdfs:comment>
    <rdfs:domain rdf:resource="http://example.org/onto/class/google_dialogflow_conversation_profile"/>
    <rdfs:range rdf:resource="http://www.w3.org/2001/XMLSchema#string"/>
  </owl:DatatypeProperty>
  <owl:DatatypeProperty rdf:about="http://example.org/onto/prop/google_dialogflow_conversation_profile_generators">
    <rdfs:label>generators</rdfs:label>
    <rdfs:comment>List of various generator resource names used in the conversation profile.</rdfs:comment>
    <rdfs:domain rdf:resource="http://example.org/onto/class/google_dialogflow_conversation_profile"/>
    <rdfs:range rdf:resource="http://www.w3.org/2001/XMLSchema#string"/>
  </owl:DatatypeProperty>
  <owl:DatatypeProperty rdf:about="http://example.org/onto/prop/google_dialogflow_conversation_profile_group_suggestion_responses">
    <rdfs:label>group_suggestion_responses</rdfs:label>
    <rdfs:comment>If groupSuggestionResponses is false, and there are multiple featureConfigs in event based suggestion or StreamingAnalyzeContent, we will try to deliver suggestions to customers as soon as we get new suggestion. Different type of suggestions based on the same context will be in separate Pub/Sub event or StreamingAnalyzeContentResponse.

If groupSuggestionResponses set to true. All the suggestions to the same participant based on the same context will be grouped into a single Pub/Sub event or StreamingAnalyzeContentResponse.</rdfs:comment>
    <rdfs:domain rdf:resource="http://example.org/onto/class/google_dialogflow_conversation_profile"/>
    <rdfs:range rdf:resource="http://www.w3.org/2001/XMLSchema#string"/>
  </owl:DatatypeProperty>
  <owl:DatatypeProperty rdf:about="http://example.org/onto/prop/google_dialogflow_conversation_profile_disable_agent_query_logging">
    <rdfs:label>disable_agent_query_logging</rdfs:label>
    <rdfs:comment>Disable the logging of search queries sent by human agents. It can prevent those queries from being stored at answer records.
This feature is only supported for types: KNOWLEDGE_SEARCH.</rdfs:comment>
    <rdfs:domain rdf:resource="http://example.org/onto/class/google_dialogflow_conversation_profile"/>
    <rdfs:range rdf:resource="http://www.w3.org/2001/XMLSchema#string"/>
  </owl:DatatypeProperty>
  <owl:DatatypeProperty rdf:about="http://example.org/onto/prop/google_dialogflow_conversation_profile_enable_conversation_augmented_query">
    <rdfs:label>enable_conversation_augmented_query</rdfs:label>
    <rdfs:comment>Enable including conversation context during query answer generation.
This feature is only supported for types: KNOWLEDGE_SEARCH.</rdfs:comment>
    <rdfs:domain rdf:resource="http://example.org/onto/class/google_dialogflow_conversation_profile"/>
    <rdfs:range rdf:resource="http://www.w3.org/2001/XMLSchema#string"/>
  </owl:DatatypeProperty>
  <owl:DatatypeProperty rdf:about="http://example.org/onto/prop/google_dialogflow_conversation_profile_enable_event_based_suggestion">
    <rdfs:label>enable_event_based_suggestion</rdfs:label>
    <rdfs:comment>Automatically iterates all participants and tries to compile suggestions.
This feature is only supported for types: ARTICLE_SUGGESTION, FAQ, DIALOGFLOW_ASSIST, KNOWLEDGE_ASSIST.</rdfs:comment>
    <rdfs:domain rdf:resource="http://example.org/onto/class/google_dialogflow_conversation_profile"/>
    <rdfs:range rdf:resource="http://www.w3.org/2001/XMLSchema#string"/>
  </owl:DatatypeProperty>
  <owl:DatatypeProperty rdf:about="http://example.org/onto/prop/google_dialogflow_conversation_profile_enable_query_suggestion_only">
    <rdfs:label>enable_query_suggestion_only</rdfs:label>
    <rdfs:comment>Enable query suggestion only.
This feature is only supported for types: KNOWLEDGE_ASSIST</rdfs:comment>
    <rdfs:domain rdf:resource="http://example.org/onto/class/google_dialogflow_conversation_profile"/>
    <rdfs:range rdf:resource="http://www.w3.org/2001/XMLSchema#string"/>
  </owl:DatatypeProperty>
  <owl:DatatypeProperty rdf:about="http://example.org/onto/prop/google_dialogflow_conversation_profile_enable_query_suggestion_when_no_answer">
    <rdfs:label>enable_query_suggestion_when_no_answer</rdfs:label>
    <rdfs:comment>Enable query suggestion even if we can't find its answer. By default, queries are suggested only if we find its answer.
This feature is only supported for types: KNOWLEDGE_ASSIST.</rdfs:comment>
    <rdfs:domain rdf:resource="http://example.org/onto/class/google_dialogflow_conversation_profile"/>
    <rdfs:range rdf:resource="http://www.w3.org/2001/XMLSchema#string"/>
  </owl:DatatypeProperty>
  <owl:DatatypeProperty rdf:about="http://example.org/onto/prop/google_dialogflow_conversation_profile_baseline_model_version">
    <rdfs:label>baseline_model_version</rdfs:label>
    <rdfs:comment>Version of current baseline model. It will be ignored if model is set. Valid versions are: Article Suggestion baseline model: - 0.9 - 1.0 (default) Summarization baseline model: - 1.0</rdfs:comment>
    <rdfs:domain rdf:resource="http://example.org/onto/class/google_dialogflow_conversation_profile"/>
    <rdfs:range rdf:resource="http://www.w3.org/2001/XMLSchema#string"/>
  </owl:DatatypeProperty>
  <owl:DatatypeProperty rdf:about="http://example.org/onto/prop/google_dialogflow_conversation_profile_model">
    <rdfs:label>model</rdfs:label>
    <rdfs:comment>Conversation model resource name. Format: projects/<Project ID>/conversationModels/<Model ID>.</rdfs:comment>
    <rdfs:domain rdf:resource="http://example.org/onto/class/google_dialogflow_conversation_profile"/>
    <rdfs:range rdf:resource="http://www.w3.org/2001/XMLSchema#string"/>
  </owl:DatatypeProperty>
  <owl:DatatypeProperty rdf:about="http://example.org/onto/prop/google_dialogflow_conversation_profile_recent_sentences_count">
    <rdfs:label>recent_sentences_count</rdfs:label>
    <rdfs:comment>Number of recent non-small-talk sentences to use as context for article and FAQ suggestion</rdfs:comment>
    <rdfs:domain rdf:resource="http://example.org/onto/class/google_dialogflow_conversation_profile"/>
    <rdfs:range rdf:resource="http://www.w3.org/2001/XMLSchema#string"/>
  </owl:DatatypeProperty>
  <owl:DatatypeProperty rdf:about="http://example.org/onto/prop/google_dialogflow_conversation_profile_confidence_threshold">
    <rdfs:label>confidence_threshold</rdfs:label>
    <rdfs:comment>Confidence threshold of query result.
This feature is only supported for types: ARTICLE_SUGGESTION, FAQ, SMART_REPLY, SMART_COMPOSE, KNOWLEDGE_SEARCH, KNOWLEDGE_ASSIST, ENTITY_EXTRACTION.</rdfs:comment>
    <rdfs:domain rdf:resource="http://example.org/onto/class/google_dialogflow_conversation_profile"/>
    <rdfs:range rdf:resource="http://www.w3.org/2001/XMLSchema#string"/>
  </owl:DatatypeProperty>
  <owl:DatatypeProperty rdf:about="http://example.org/onto/prop/google_dialogflow_conversation_profile_max_results">
    <rdfs:label>max_results</rdfs:label>
    <rdfs:comment>Maximum number of results to return.</rdfs:comment>
    <rdfs:domain rdf:resource="http://example.org/onto/class/google_dialogflow_conversation_profile"/>
    <rdfs:range rdf:resource="http://www.w3.org/2001/XMLSchema#string"/>
  </owl:DatatypeProperty>
  <owl:DatatypeProperty rdf:about="http://example.org/onto/prop/google_dialogflow_conversation_profile_drop_handoff_messages">
    <rdfs:label>drop_handoff_messages</rdfs:label>
    <rdfs:comment>If set to true, the last message from virtual agent (hand off message) and the message before it (trigger message of hand off) are dropped.</rdfs:comment>
    <rdfs:domain rdf:resource="http://example.org/onto/class/google_dialogflow_conversation_profile"/>
    <rdfs:range rdf:resource="http://www.w3.org/2001/XMLSchema#string"/>
  </owl:DatatypeProperty>
  <owl:DatatypeProperty rdf:about="http://example.org/onto/prop/google_dialogflow_conversation_profile_drop_ivr_messages">
    <rdfs:label>drop_ivr_messages</rdfs:label>
    <rdfs:comment>If set to true, all messages from ivr stage are dropped.</rdfs:comment>
    <rdfs:domain rdf:resource="http://example.org/onto/class/google_dialogflow_conversation_profile"/>
    <rdfs:range rdf:resource="http://www.w3.org/2001/XMLSchema#string"/>
  </owl:DatatypeProperty>
  <owl:DatatypeProperty rdf:about="http://example.org/onto/prop/google_dialogflow_conversation_profile_drop_virtual_agent_messages">
    <rdfs:label>drop_virtual_agent_messages</rdfs:label>
    <rdfs:comment>If set to true, all messages from virtual agent are dropped.</rdfs:comment>
    <rdfs:domain rdf:resource="http://example.org/onto/class/google_dialogflow_conversation_profile"/>
    <rdfs:range rdf:resource="http://www.w3.org/2001/XMLSchema#string"/>
  </owl:DatatypeProperty>
  <owl:DatatypeProperty rdf:about="http://example.org/onto/prop/google_dialogflow_conversation_profile_agent">
    <rdfs:label>agent</rdfs:label>
    <rdfs:comment>he name of a Dialogflow virtual agent used for end user side intent detection and suggestion. Format: projects/<Project ID>/locations/<Location ID>/agent.</rdfs:comment>
    <rdfs:domain rdf:resource="http://example.org/onto/class/google_dialogflow_conversation_profile"/>
    <rdfs:range rdf:resource="http://www.w3.org/2001/XMLSchema#string"/>
  </owl:DatatypeProperty>
  <owl:DatatypeProperty rdf:about="http://example.org/onto/prop/google_dialogflow_conversation_profile_agent">
    <rdfs:label>agent</rdfs:label>
    <rdfs:comment>The name of a dialogflow virtual agent used for intent detection and suggestion triggered by human agent. Format: projects/<Project ID>/locations/<Location ID>/agent.</rdfs:comment>
    <rdfs:domain rdf:resource="http://example.org/onto/class/google_dialogflow_conversation_profile"/>
    <rdfs:range rdf:resource="http://www.w3.org/2001/XMLSchema#string"/>
  </owl:DatatypeProperty>
  <owl:DatatypeProperty rdf:about="http://example.org/onto/prop/google_dialogflow_conversation_profile_section_types">
    <rdfs:label>section_types</rdfs:label>
    <rdfs:comment>The selected sections chosen to return when requesting a summary of a conversation
If not provided the default selection will be "{SITUATION, ACTION, RESULT}". Possible values: ["SECTION_TYPE_UNSPECIFIED", "SITUATION", "ACTION", "RESOLUTION", "REASON_FOR_CANCELLATION", "CUSTOMER_SATISFACTION", "ENTITIES"]</rdfs:comment>
    <rdfs:domain rdf:resource="http://example.org/onto/class/google_dialogflow_conversation_profile"/>
    <rdfs:range rdf:resource="http://www.w3.org/2001/XMLSchema#string"/>
  </owl:DatatypeProperty>
  <owl:DatatypeProperty rdf:about="http://example.org/onto/prop/google_dialogflow_conversation_profile_type">
    <rdfs:label>type</rdfs:label>
    <rdfs:comment>Type of Human Agent Assistant API feature to request.</rdfs:comment>
    <rdfs:domain rdf:resource="http://example.org/onto/class/google_dialogflow_conversation_profile"/>
    <rdfs:range rdf:resource="http://www.w3.org/2001/XMLSchema#string"/>
  </owl:DatatypeProperty>
  <owl:DatatypeProperty rdf:about="http://example.org/onto/prop/google_dialogflow_conversation_profile_no_small_talk">
    <rdfs:label>no_small_talk</rdfs:label>
    <rdfs:comment>Do not trigger if last utterance is small talk.</rdfs:comment>
    <rdfs:domain rdf:resource="http://example.org/onto/class/google_dialogflow_conversation_profile"/>
    <rdfs:range rdf:resource="http://www.w3.org/2001/XMLSchema#string"/>
  </owl:DatatypeProperty>
  <owl:DatatypeProperty rdf:about="http://example.org/onto/prop/google_dialogflow_conversation_profile_only_end_user">
    <rdfs:label>only_end_user</rdfs:label>
    <rdfs:comment>Only trigger suggestion if participant role of last utterance is END_USER.</rdfs:comment>
    <rdfs:domain rdf:resource="http://example.org/onto/class/google_dialogflow_conversation_profile"/>
    <rdfs:range rdf:resource="http://www.w3.org/2001/XMLSchema#string"/>
  </owl:DatatypeProperty>
  <owl:DatatypeProperty rdf:about="http://example.org/onto/prop/google_dialogflow_conversation_profile_enable_entity_extraction">
    <rdfs:label>enable_entity_extraction</rdfs:label>
    <rdfs:comment>Enable entity extraction in conversation messages on agent assist stage.</rdfs:comment>
    <rdfs:domain rdf:resource="http://example.org/onto/class/google_dialogflow_conversation_profile"/>
    <rdfs:range rdf:resource="http://www.w3.org/2001/XMLSchema#string"/>
  </owl:DatatypeProperty>
  <owl:DatatypeProperty rdf:about="http://example.org/onto/prop/google_dialogflow_conversation_profile_enable_sentiment_analysis">
    <rdfs:label>enable_sentiment_analysis</rdfs:label>
    <rdfs:comment>Enable sentiment analysis in conversation messages on agent assist stage. Sentiment analysis inspects user input and identifies the prevailing subjective opinion, especially to determine a user's attitude as positive, negative, or neutral.</rdfs:comment>
    <rdfs:domain rdf:resource="http://example.org/onto/class/google_dialogflow_conversation_profile"/>
    <rdfs:range rdf:resource="http://www.w3.org/2001/XMLSchema#string"/>
  </owl:DatatypeProperty>
  <owl:DatatypeProperty rdf:about="http://example.org/onto/prop/google_dialogflow_conversation_profile_message_format">
    <rdfs:label>message_format</rdfs:label>
    <rdfs:comment>Format of the message Possible values: ["MESSAGE_FORMAT_UNSPECIFIED", "PROTO", "JSON"]</rdfs:comment>
    <rdfs:domain rdf:resource="http://example.org/onto/class/google_dialogflow_conversation_profile"/>
    <rdfs:range rdf:resource="http://www.w3.org/2001/XMLSchema#string"/>
  </owl:DatatypeProperty>
  <owl:DatatypeProperty rdf:about="http://example.org/onto/prop/google_dialogflow_conversation_profile_topic">
    <rdfs:label>topic</rdfs:label>
    <rdfs:comment>Name of the Pub/Sub topic to publish conversation events</rdfs:comment>
    <rdfs:domain rdf:resource="http://example.org/onto/class/google_dialogflow_conversation_profile"/>
    <rdfs:range rdf:resource="http://www.w3.org/2001/XMLSchema#string"/>
  </owl:DatatypeProperty>
  <owl:DatatypeProperty rdf:about="http://example.org/onto/prop/google_dialogflow_conversation_profile_account_number">
    <rdfs:label>account_number</rdfs:label>
    <rdfs:comment>Account number of the LivePerson account to connect.</rdfs:comment>
    <rdfs:domain rdf:resource="http://example.org/onto/class/google_dialogflow_conversation_profile"/>
    <rdfs:range rdf:resource="http://www.w3.org/2001/XMLSchema#string"/>
  </owl:DatatypeProperty>
  <owl:DatatypeProperty rdf:about="http://example.org/onto/prop/google_dialogflow_conversation_profile_enable_stackdriver_logging">
    <rdfs:label>enable_stackdriver_logging</rdfs:label>
    <rdfs:comment>Whether to log conversation events</rdfs:comment>
    <rdfs:domain rdf:resource="http://example.org/onto/class/google_dialogflow_conversation_profile"/>
    <rdfs:range rdf:resource="http://www.w3.org/2001/XMLSchema#string"/>
  </owl:DatatypeProperty>
  <owl:DatatypeProperty rdf:about="http://example.org/onto/prop/google_dialogflow_conversation_profile_message_format">
    <rdfs:label>message_format</rdfs:label>
    <rdfs:comment>Format of the message Possible values: ["MESSAGE_FORMAT_UNSPECIFIED", "PROTO", "JSON"]</rdfs:comment>
    <rdfs:domain rdf:resource="http://example.org/onto/class/google_dialogflow_conversation_profile"/>
    <rdfs:range rdf:resource="http://www.w3.org/2001/XMLSchema#string"/>
  </owl:DatatypeProperty>
  <owl:DatatypeProperty rdf:about="http://example.org/onto/prop/google_dialogflow_conversation_profile_topic">
    <rdfs:label>topic</rdfs:label>
    <rdfs:comment>Name of the Pub/Sub topic to publish conversation events</rdfs:comment>
    <rdfs:domain rdf:resource="http://example.org/onto/class/google_dialogflow_conversation_profile"/>
    <rdfs:range rdf:resource="http://www.w3.org/2001/XMLSchema#string"/>
  </owl:DatatypeProperty>
  <owl:DatatypeProperty rdf:about="http://example.org/onto/prop/google_dialogflow_conversation_profile_message_format">
    <rdfs:label>message_format</rdfs:label>
    <rdfs:comment>Format of message. Possible values: ["MESSAGE_FORMAT_UNSPECIFIED", "PROTO", "JSON"]</rdfs:comment>
    <rdfs:domain rdf:resource="http://example.org/onto/class/google_dialogflow_conversation_profile"/>
    <rdfs:range rdf:resource="http://www.w3.org/2001/XMLSchema#string"/>
  </owl:DatatypeProperty>
  <owl:DatatypeProperty rdf:about="http://example.org/onto/prop/google_dialogflow_conversation_profile_topic">
    <rdfs:label>topic</rdfs:label>
    <rdfs:comment>Name of the Pub/Sub topic to publish conversation events like CONVERSATION_STARTED as serialized ConversationEvent protos.
For telephony integration to receive notification, make sure either this topic is in the same project as the conversation or you grant service-<Conversation Project Number>@gcp-sa-dialogflow.iam.gserviceaccount.com the Dialogflow Service Agent role in the topic project.
For chat integration to receive notification, make sure API caller has been granted the Dialogflow Service Agent role for the topic.
Format: projects/<Project ID>/locations/<Location ID>/topics/<Topic ID>.</rdfs:comment>
    <rdfs:domain rdf:resource="http://example.org/onto/class/google_dialogflow_conversation_profile"/>
    <rdfs:range rdf:resource="http://www.w3.org/2001/XMLSchema#string"/>
  </owl:DatatypeProperty>
  <owl:DatatypeProperty rdf:about="http://example.org/onto/prop/google_dialogflow_conversation_profile_message_format">
    <rdfs:label>message_format</rdfs:label>
    <rdfs:comment>Format of the message Possible values: ["MESSAGE_FORMAT_UNSPECIFIED", "PROTO", "JSON"]</rdfs:comment>
    <rdfs:domain rdf:resource="http://example.org/onto/class/google_dialogflow_conversation_profile"/>
    <rdfs:range rdf:resource="http://www.w3.org/2001/XMLSchema#string"/>
  </owl:DatatypeProperty>
  <owl:DatatypeProperty rdf:about="http://example.org/onto/prop/google_dialogflow_conversation_profile_topic">
    <rdfs:label>topic</rdfs:label>
    <rdfs:comment>Name of the Pub/Sub topic to publish conversation events</rdfs:comment>
    <rdfs:domain rdf:resource="http://example.org/onto/class/google_dialogflow_conversation_profile"/>
    <rdfs:range rdf:resource="http://www.w3.org/2001/XMLSchema#string"/>
  </owl:DatatypeProperty>
  <owl:DatatypeProperty rdf:about="http://example.org/onto/prop/google_dialogflow_conversation_profile_audio_encoding">
    <rdfs:label>audio_encoding</rdfs:label>
    <rdfs:comment>Audio encoding of the audio content to process. Possible values: ["AUDIO_ENCODING_UNSPECIFIED", "AUDIO_ENCODING_LINEAR_16", "AUDIO_ENCODING_FLAC", "AUDIO_ENCODING_MULAW", "AUDIO_ENCODING_AMR", "AUDIO_ENCODING_AMR_WB", "AUDIO_ENCODING_OGG_OPUS", "AUDIOENCODING_SPEEX_WITH_HEADER_BYTE"]</rdfs:comment>
    <rdfs:domain rdf:resource="http://example.org/onto/class/google_dialogflow_conversation_profile"/>
    <rdfs:range rdf:resource="http://www.w3.org/2001/XMLSchema#string"/>
  </owl:DatatypeProperty>
  <owl:DatatypeProperty rdf:about="http://example.org/onto/prop/google_dialogflow_conversation_profile_enable_word_info">
    <rdfs:label>enable_word_info</rdfs:label>
    <rdfs:comment>If true, Dialogflow returns SpeechWordInfo in StreamingRecognitionResult with information about the recognized speech words.</rdfs:comment>
    <rdfs:domain rdf:resource="http://example.org/onto/class/google_dialogflow_conversation_profile"/>
    <rdfs:range rdf:resource="http://www.w3.org/2001/XMLSchema#string"/>
  </owl:DatatypeProperty>
  <owl:DatatypeProperty rdf:about="http://example.org/onto/prop/google_dialogflow_conversation_profile_language_code">
    <rdfs:label>language_code</rdfs:label>
    <rdfs:comment>The language of the supplied audio.</rdfs:comment>
    <rdfs:domain rdf:resource="http://example.org/onto/class/google_dialogflow_conversation_profile"/>
    <rdfs:range rdf:resource="http://www.w3.org/2001/XMLSchema#string"/>
  </owl:DatatypeProperty>
  <owl:DatatypeProperty rdf:about="http://example.org/onto/prop/google_dialogflow_conversation_profile_model">
    <rdfs:label>model</rdfs:label>
    <rdfs:comment>Which Speech model to select.
Leave this field unspecified to use Agent Speech settings for model selection.</rdfs:comment>
    <rdfs:domain rdf:resource="http://example.org/onto/class/google_dialogflow_conversation_profile"/>
    <rdfs:range rdf:resource="http://www.w3.org/2001/XMLSchema#string"/>
  </owl:DatatypeProperty>
  <owl:DatatypeProperty rdf:about="http://example.org/onto/prop/google_dialogflow_conversation_profile_sample_rate_hertz">
    <rdfs:label>sample_rate_hertz</rdfs:label>
    <rdfs:comment>Sample rate (in Hertz) of the audio content sent in the query.</rdfs:comment>
    <rdfs:domain rdf:resource="http://example.org/onto/class/google_dialogflow_conversation_profile"/>
    <rdfs:range rdf:resource="http://www.w3.org/2001/XMLSchema#string"/>
  </owl:DatatypeProperty>
  <owl:DatatypeProperty rdf:about="http://example.org/onto/prop/google_dialogflow_conversation_profile_speech_model_variant">
    <rdfs:label>speech_model_variant</rdfs:label>
    <rdfs:comment>The speech model used in speech to text. Possible values: ["SPEECH_MODEL_VARIANT_UNSPECIFIED", "USE_BEST_AVAILABLE", "USE_STANDARD", "USE_ENHANCED"]</rdfs:comment>
    <rdfs:domain rdf:resource="http://example.org/onto/class/google_dialogflow_conversation_profile"/>
    <rdfs:range rdf:resource="http://www.w3.org/2001/XMLSchema#string"/>
  </owl:DatatypeProperty>
  <owl:DatatypeProperty rdf:about="http://example.org/onto/prop/google_dialogflow_conversation_profile_use_timeout_based_endpointing">
    <rdfs:label>use_timeout_based_endpointing</rdfs:label>
    <rdfs:comment>Use timeout based endpointing, interpreting endpointer sensitivy as seconds of timeout value.</rdfs:comment>
    <rdfs:domain rdf:resource="http://example.org/onto/class/google_dialogflow_conversation_profile"/>
    <rdfs:range rdf:resource="http://www.w3.org/2001/XMLSchema#string"/>
  </owl:DatatypeProperty>
  <owl:DatatypeProperty rdf:about="http://example.org/onto/prop/google_dialogflow_conversation_profile_create">
    <rdfs:label>create</rdfs:label>
    <rdfs:domain rdf:resource="http://example.org/onto/class/google_dialogflow_conversation_profile"/>
    <rdfs:range rdf:resource="http://www.w3.org/2001/XMLSchema#string"/>
  </owl:DatatypeProperty>
  <owl:DatatypeProperty rdf:about="http://example.org/onto/prop/google_dialogflow_conversation_profile_delete">
    <rdfs:label>delete</rdfs:label>
    <rdfs:domain rdf:resource="http://example.org/onto/class/google_dialogflow_conversation_profile"/>
    <rdfs:range rdf:resource="http://www.w3.org/2001/XMLSchema#string"/>
  </owl:DatatypeProperty>
  <owl:DatatypeProperty rdf:about="http://example.org/onto/prop/google_dialogflow_conversation_profile_update">
    <rdfs:label>update</rdfs:label>
    <rdfs:domain rdf:resource="http://example.org/onto/class/google_dialogflow_conversation_profile"/>
    <rdfs:range rdf:resource="http://www.w3.org/2001/XMLSchema#string"/>
  </owl:DatatypeProperty>
  <owl:DatatypeProperty rdf:about="http://example.org/onto/prop/google_dialogflow_conversation_profile_effects_profile_id">
    <rdfs:label>effects_profile_id</rdfs:label>
    <rdfs:comment>An identifier which selects 'audio effects' profiles that are applied on (post synthesized) text to speech. Effects are applied on top of each other in the order they are given.</rdfs:comment>
    <rdfs:domain rdf:resource="http://example.org/onto/class/google_dialogflow_conversation_profile"/>
    <rdfs:range rdf:resource="http://www.w3.org/2001/XMLSchema#string"/>
  </owl:DatatypeProperty>
  <owl:DatatypeProperty rdf:about="http://example.org/onto/prop/google_dialogflow_conversation_profile_pitch">
    <rdfs:label>pitch</rdfs:label>
    <rdfs:comment>Speaking pitch, in the range [-20.0, 20.0]. 20 means increase 20 semitones from the original pitch. -20 means decrease 20 semitones from the original pitch.</rdfs:comment>
    <rdfs:domain rdf:resource="http://example.org/onto/class/google_dialogflow_conversation_profile"/>
    <rdfs:range rdf:resource="http://www.w3.org/2001/XMLSchema#string"/>
  </owl:DatatypeProperty>
  <owl:DatatypeProperty rdf:about="http://example.org/onto/prop/google_dialogflow_conversation_profile_speaking_rate">
    <rdfs:label>speaking_rate</rdfs:label>
    <rdfs:comment>Speaking rate/speed, in the range [0.25, 4.0].</rdfs:comment>
    <rdfs:domain rdf:resource="http://example.org/onto/class/google_dialogflow_conversation_profile"/>
    <rdfs:range rdf:resource="http://www.w3.org/2001/XMLSchema#string"/>
  </owl:DatatypeProperty>
  <owl:DatatypeProperty rdf:about="http://example.org/onto/prop/google_dialogflow_conversation_profile_volume_gain_db">
    <rdfs:label>volume_gain_db</rdfs:label>
    <rdfs:comment>Volume gain (in dB) of the normal native volume supported by the specific voice.</rdfs:comment>
    <rdfs:domain rdf:resource="http://example.org/onto/class/google_dialogflow_conversation_profile"/>
    <rdfs:range rdf:resource="http://www.w3.org/2001/XMLSchema#string"/>
  </owl:DatatypeProperty>
  <owl:DatatypeProperty rdf:about="http://example.org/onto/prop/google_dialogflow_conversation_profile_name">
    <rdfs:label>name</rdfs:label>
    <rdfs:comment>The name of the voice.</rdfs:comment>
    <rdfs:domain rdf:resource="http://example.org/onto/class/google_dialogflow_conversation_profile"/>
    <rdfs:range rdf:resource="http://www.w3.org/2001/XMLSchema#string"/>
  </owl:DatatypeProperty>
  <owl:DatatypeProperty rdf:about="http://example.org/onto/prop/google_dialogflow_conversation_profile_ssml_gender">
    <rdfs:label>ssml_gender</rdfs:label>
    <rdfs:comment>The preferred gender of the voice. Possible values: ["SSML_VOICE_GENDER_UNSPECIFIED", "SSML_VOICE_GENDER_MALE", "SSML_VOICE_GENDER_FEMALE", "SSML_VOICE_GENDER_NEUTRAL"]</rdfs:comment>
    <rdfs:domain rdf:resource="http://example.org/onto/class/google_dialogflow_conversation_profile"/>
    <rdfs:range rdf:resource="http://www.w3.org/2001/XMLSchema#string"/>
  </owl:DatatypeProperty>
</rdf:RDF>
