<?xml version="1.0" encoding="UTF-8"?>
<rdf:RDF
  xmlns:rdf="http://www.w3.org/1999/02/22-rdf-syntax-ns#"
  xmlns:rdfs="http://www.w3.org/2000/01/rdf-schema#"
  xmlns:owl="http://www.w3.org/2002/07/owl#"
  xmlns:xsd="http://www.w3.org/2001/XMLSchema#"
  xml:base="http://example.org/onto/">
  <owl:Class rdf:about="http://example.org/onto/class/google_container_azure_node_pool">
    <rdfs:label>google_container_azure_node_pool</rdfs:label>
    <rdfs:comment>#
#     ***     AUTO GENERATED CODE    ***    Type: DCL     ***
#
# ----------------------------------------------------------------------------
#
#     This file is managed by Magic Modules (https:#github.com/GoogleCloudPlatform/magic-modules)
#     and is based on the DCL (https:#github.com/GoogleCloudPlatform/declarative-resource-client-library).
#     Changes will need to be made to the DCL or Magic Modules instead of here.
#
#     We are not currently able to accept contributions to this file. If changes
#     are required, please file an issue at https:#github.com/hashicorp/terraform-provider-google/issues/new/choose
#
# ----------------------------------------------------------------------------
subcategory: "ContainerAzure"
description: |-
  An Anthos node pool running on Azure.
---</rdfs:comment>
  </owl:Class>
  <owl:DatatypeProperty rdf:about="http://example.org/onto/prop/google_container_azure_node_pool_annotations">
    <rdfs:label>annotations</rdfs:label>
    <rdfs:comment>Optional. Annotations on the node pool. This field has the same restrictions as Kubernetes annotations. The total size of all keys and values combined is limited to 256k. Keys can have 2 segments: prefix (optional) and name (required), separated by a slash (/). Prefix must be a DNS subdomain. Name must be 63 characters or less, begin and end with alphanumerics, with dashes (-), underscores (_), dots (.), and alphanumerics between.

**Note**: This field is non-authoritative, and will only manage the annotations present in your configuration.
Please refer to the field `effective_annotations` for all of the annotations present on the resource.</rdfs:comment>
    <rdfs:domain rdf:resource="http://example.org/onto/class/google_container_azure_node_pool"/>
    <rdfs:range rdf:resource="http://www.w3.org/2001/XMLSchema#string"/>
  </owl:DatatypeProperty>
  <owl:DatatypeProperty rdf:about="http://example.org/onto/prop/google_container_azure_node_pool_azure_availability_zone">
    <rdfs:label>azure_availability_zone</rdfs:label>
    <rdfs:comment>Optional. The Azure availability zone of the nodes in this nodepool. When unspecified, it defaults to `1`.</rdfs:comment>
    <rdfs:domain rdf:resource="http://example.org/onto/class/google_container_azure_node_pool"/>
    <rdfs:range rdf:resource="http://www.w3.org/2001/XMLSchema#string"/>
  </owl:DatatypeProperty>
  <owl:DatatypeProperty rdf:about="http://example.org/onto/prop/google_container_azure_node_pool_cluster">
    <rdfs:label>cluster</rdfs:label>
    <rdfs:comment>The azureCluster for the resource</rdfs:comment>
    <rdfs:domain rdf:resource="http://example.org/onto/class/google_container_azure_node_pool"/>
    <rdfs:range rdf:resource="http://www.w3.org/2001/XMLSchema#string"/>
  </owl:DatatypeProperty>
  <owl:DatatypeProperty rdf:about="http://example.org/onto/prop/google_container_azure_node_pool_create_time">
    <rdfs:label>create_time</rdfs:label>
    <rdfs:comment>Output only. The time at which this node pool was created.</rdfs:comment>
    <rdfs:domain rdf:resource="http://example.org/onto/class/google_container_azure_node_pool"/>
    <rdfs:range rdf:resource="http://www.w3.org/2001/XMLSchema#string"/>
  </owl:DatatypeProperty>
  <owl:DatatypeProperty rdf:about="http://example.org/onto/prop/google_container_azure_node_pool_effective_annotations">
    <rdfs:label>effective_annotations</rdfs:label>
    <rdfs:comment>All of annotations (key/value pairs) present on the resource in GCP, including the annotations configured through Terraform, other clients and services.</rdfs:comment>
    <rdfs:domain rdf:resource="http://example.org/onto/class/google_container_azure_node_pool"/>
    <rdfs:range rdf:resource="http://www.w3.org/2001/XMLSchema#string"/>
  </owl:DatatypeProperty>
  <owl:DatatypeProperty rdf:about="http://example.org/onto/prop/google_container_azure_node_pool_etag">
    <rdfs:label>etag</rdfs:label>
    <rdfs:comment>Allows clients to perform consistent read-modify-writes through optimistic concurrency control. May be sent on update and delete requests to ensure the client has an up-to-date value before proceeding.</rdfs:comment>
    <rdfs:domain rdf:resource="http://example.org/onto/class/google_container_azure_node_pool"/>
    <rdfs:range rdf:resource="http://www.w3.org/2001/XMLSchema#string"/>
  </owl:DatatypeProperty>
  <owl:DatatypeProperty rdf:about="http://example.org/onto/prop/google_container_azure_node_pool_id">
    <rdfs:label>id</rdfs:label>
    <rdfs:domain rdf:resource="http://example.org/onto/class/google_container_azure_node_pool"/>
    <rdfs:range rdf:resource="http://www.w3.org/2001/XMLSchema#string"/>
  </owl:DatatypeProperty>
  <owl:DatatypeProperty rdf:about="http://example.org/onto/prop/google_container_azure_node_pool_location">
    <rdfs:label>location</rdfs:label>
    <rdfs:comment>The location for the resource</rdfs:comment>
    <rdfs:domain rdf:resource="http://example.org/onto/class/google_container_azure_node_pool"/>
    <rdfs:range rdf:resource="http://www.w3.org/2001/XMLSchema#string"/>
  </owl:DatatypeProperty>
  <owl:DatatypeProperty rdf:about="http://example.org/onto/prop/google_container_azure_node_pool_name">
    <rdfs:label>name</rdfs:label>
    <rdfs:comment>The name of this resource.</rdfs:comment>
    <rdfs:domain rdf:resource="http://example.org/onto/class/google_container_azure_node_pool"/>
    <rdfs:range rdf:resource="http://www.w3.org/2001/XMLSchema#string"/>
  </owl:DatatypeProperty>
  <owl:DatatypeProperty rdf:about="http://example.org/onto/prop/google_container_azure_node_pool_project">
    <rdfs:label>project</rdfs:label>
    <rdfs:comment>The project for the resource</rdfs:comment>
    <rdfs:domain rdf:resource="http://example.org/onto/class/google_container_azure_node_pool"/>
    <rdfs:range rdf:resource="http://www.w3.org/2001/XMLSchema#string"/>
  </owl:DatatypeProperty>
  <owl:DatatypeProperty rdf:about="http://example.org/onto/prop/google_container_azure_node_pool_reconciling">
    <rdfs:label>reconciling</rdfs:label>
    <rdfs:comment>Output only. If set, there are currently pending changes to the node pool.</rdfs:comment>
    <rdfs:domain rdf:resource="http://example.org/onto/class/google_container_azure_node_pool"/>
    <rdfs:range rdf:resource="http://www.w3.org/2001/XMLSchema#string"/>
  </owl:DatatypeProperty>
  <owl:DatatypeProperty rdf:about="http://example.org/onto/prop/google_container_azure_node_pool_state">
    <rdfs:label>state</rdfs:label>
    <rdfs:comment>Output only. The current state of the node pool. Possible values: STATE_UNSPECIFIED, PROVISIONING, RUNNING, RECONCILING, STOPPING, ERROR, DEGRADED</rdfs:comment>
    <rdfs:domain rdf:resource="http://example.org/onto/class/google_container_azure_node_pool"/>
    <rdfs:range rdf:resource="http://www.w3.org/2001/XMLSchema#string"/>
  </owl:DatatypeProperty>
  <owl:DatatypeProperty rdf:about="http://example.org/onto/prop/google_container_azure_node_pool_subnet_id">
    <rdfs:label>subnet_id</rdfs:label>
    <rdfs:comment>The ARM ID of the subnet where the node pool VMs run. Make sure it's a subnet under the virtual network in the cluster configuration.</rdfs:comment>
    <rdfs:domain rdf:resource="http://example.org/onto/class/google_container_azure_node_pool"/>
    <rdfs:range rdf:resource="http://www.w3.org/2001/XMLSchema#string"/>
  </owl:DatatypeProperty>
  <owl:DatatypeProperty rdf:about="http://example.org/onto/prop/google_container_azure_node_pool_uid">
    <rdfs:label>uid</rdfs:label>
    <rdfs:comment>Output only. A globally unique identifier for the node pool.</rdfs:comment>
    <rdfs:domain rdf:resource="http://example.org/onto/class/google_container_azure_node_pool"/>
    <rdfs:range rdf:resource="http://www.w3.org/2001/XMLSchema#string"/>
  </owl:DatatypeProperty>
  <owl:DatatypeProperty rdf:about="http://example.org/onto/prop/google_container_azure_node_pool_update_time">
    <rdfs:label>update_time</rdfs:label>
    <rdfs:comment>Output only. The time at which this node pool was last updated.</rdfs:comment>
    <rdfs:domain rdf:resource="http://example.org/onto/class/google_container_azure_node_pool"/>
    <rdfs:range rdf:resource="http://www.w3.org/2001/XMLSchema#string"/>
  </owl:DatatypeProperty>
  <owl:DatatypeProperty rdf:about="http://example.org/onto/prop/google_container_azure_node_pool_version">
    <rdfs:label>version</rdfs:label>
    <rdfs:comment>The Kubernetes version (e.g. `1.19.10-gke.1000`) running on this node pool.</rdfs:comment>
    <rdfs:domain rdf:resource="http://example.org/onto/class/google_container_azure_node_pool"/>
    <rdfs:range rdf:resource="http://www.w3.org/2001/XMLSchema#string"/>
  </owl:DatatypeProperty>
  <owl:DatatypeProperty rdf:about="http://example.org/onto/prop/google_container_azure_node_pool_max_node_count">
    <rdfs:label>max_node_count</rdfs:label>
    <rdfs:comment>Maximum number of nodes in the node pool. Must be >= min_node_count.</rdfs:comment>
    <rdfs:domain rdf:resource="http://example.org/onto/class/google_container_azure_node_pool"/>
    <rdfs:range rdf:resource="http://www.w3.org/2001/XMLSchema#string"/>
  </owl:DatatypeProperty>
  <owl:DatatypeProperty rdf:about="http://example.org/onto/prop/google_container_azure_node_pool_min_node_count">
    <rdfs:label>min_node_count</rdfs:label>
    <rdfs:comment>Minimum number of nodes in the node pool. Must be >= 1 and <= max_node_count.</rdfs:comment>
    <rdfs:domain rdf:resource="http://example.org/onto/class/google_container_azure_node_pool"/>
    <rdfs:range rdf:resource="http://www.w3.org/2001/XMLSchema#string"/>
  </owl:DatatypeProperty>
  <owl:DatatypeProperty rdf:about="http://example.org/onto/prop/google_container_azure_node_pool_labels">
    <rdfs:label>labels</rdfs:label>
    <rdfs:comment>Optional. The initial labels assigned to nodes of this node pool. An object containing a list of "key": value pairs. Example: { "name": "wrench", "mass": "1.3kg", "count": "3" }.</rdfs:comment>
    <rdfs:domain rdf:resource="http://example.org/onto/class/google_container_azure_node_pool"/>
    <rdfs:range rdf:resource="http://www.w3.org/2001/XMLSchema#string"/>
  </owl:DatatypeProperty>
  <owl:DatatypeProperty rdf:about="http://example.org/onto/prop/google_container_azure_node_pool_tags">
    <rdfs:label>tags</rdfs:label>
    <rdfs:comment>Optional. A set of tags to apply to all underlying Azure resources for this node pool. This currently only includes Virtual Machine Scale Sets. Specify at most 50 pairs containing alphanumerics, spaces, and symbols (.+-=_:@/). Keys can be up to 127 Unicode characters. Values can be up to 255 Unicode characters.</rdfs:comment>
    <rdfs:domain rdf:resource="http://example.org/onto/class/google_container_azure_node_pool"/>
    <rdfs:range rdf:resource="http://www.w3.org/2001/XMLSchema#string"/>
  </owl:DatatypeProperty>
  <owl:DatatypeProperty rdf:about="http://example.org/onto/prop/google_container_azure_node_pool_vm_size">
    <rdfs:label>vm_size</rdfs:label>
    <rdfs:comment>Optional. The Azure VM size name. Example: `Standard_DS2_v2`. See (/anthos/clusters/docs/azure/reference/supported-vms) for options. When unspecified, it defaults to `Standard_DS2_v2`.</rdfs:comment>
    <rdfs:domain rdf:resource="http://example.org/onto/class/google_container_azure_node_pool"/>
    <rdfs:range rdf:resource="http://www.w3.org/2001/XMLSchema#string"/>
  </owl:DatatypeProperty>
  <owl:DatatypeProperty rdf:about="http://example.org/onto/prop/google_container_azure_node_pool_resource_group_id">
    <rdfs:label>resource_group_id</rdfs:label>
    <rdfs:comment>The ARM ID the of the resource group containing proxy keyvault. Resource group ids are formatted as `/subscriptions/<subscription-id>/resourceGroups/<resource-group-name>`</rdfs:comment>
    <rdfs:domain rdf:resource="http://example.org/onto/class/google_container_azure_node_pool"/>
    <rdfs:range rdf:resource="http://www.w3.org/2001/XMLSchema#string"/>
  </owl:DatatypeProperty>
  <owl:DatatypeProperty rdf:about="http://example.org/onto/prop/google_container_azure_node_pool_secret_id">
    <rdfs:label>secret_id</rdfs:label>
    <rdfs:comment>The URL the of the proxy setting secret with its version. Secret ids are formatted as `https:<key-vault-name>.vault.azure.net/secrets/<secret-name>/<secret-version>`.</rdfs:comment>
    <rdfs:domain rdf:resource="http://example.org/onto/class/google_container_azure_node_pool"/>
    <rdfs:range rdf:resource="http://www.w3.org/2001/XMLSchema#string"/>
  </owl:DatatypeProperty>
  <owl:DatatypeProperty rdf:about="http://example.org/onto/prop/google_container_azure_node_pool_size_gib">
    <rdfs:label>size_gib</rdfs:label>
    <rdfs:comment>Optional. The size of the disk, in GiBs. When unspecified, a default value is provided. See the specific reference in the parent resource.</rdfs:comment>
    <rdfs:domain rdf:resource="http://example.org/onto/class/google_container_azure_node_pool"/>
    <rdfs:range rdf:resource="http://www.w3.org/2001/XMLSchema#string"/>
  </owl:DatatypeProperty>
  <owl:DatatypeProperty rdf:about="http://example.org/onto/prop/google_container_azure_node_pool_authorized_key">
    <rdfs:label>authorized_key</rdfs:label>
    <rdfs:comment>The SSH public key data for VMs managed by Anthos. This accepts the authorized_keys file format used in OpenSSH according to the sshd(8) manual page.</rdfs:comment>
    <rdfs:domain rdf:resource="http://example.org/onto/class/google_container_azure_node_pool"/>
    <rdfs:range rdf:resource="http://www.w3.org/2001/XMLSchema#string"/>
  </owl:DatatypeProperty>
  <owl:DatatypeProperty rdf:about="http://example.org/onto/prop/google_container_azure_node_pool_auto_repair">
    <rdfs:label>auto_repair</rdfs:label>
    <rdfs:comment>Optional. Whether or not the nodes will be automatically repaired.</rdfs:comment>
    <rdfs:domain rdf:resource="http://example.org/onto/class/google_container_azure_node_pool"/>
    <rdfs:range rdf:resource="http://www.w3.org/2001/XMLSchema#string"/>
  </owl:DatatypeProperty>
  <owl:DatatypeProperty rdf:about="http://example.org/onto/prop/google_container_azure_node_pool_max_pods_per_node">
    <rdfs:label>max_pods_per_node</rdfs:label>
    <rdfs:comment>The maximum number of pods to schedule on a single node.</rdfs:comment>
    <rdfs:domain rdf:resource="http://example.org/onto/class/google_container_azure_node_pool"/>
    <rdfs:range rdf:resource="http://www.w3.org/2001/XMLSchema#string"/>
  </owl:DatatypeProperty>
  <owl:DatatypeProperty rdf:about="http://example.org/onto/prop/google_container_azure_node_pool_create">
    <rdfs:label>create</rdfs:label>
    <rdfs:domain rdf:resource="http://example.org/onto/class/google_container_azure_node_pool"/>
    <rdfs:range rdf:resource="http://www.w3.org/2001/XMLSchema#string"/>
  </owl:DatatypeProperty>
  <owl:DatatypeProperty rdf:about="http://example.org/onto/prop/google_container_azure_node_pool_delete">
    <rdfs:label>delete</rdfs:label>
    <rdfs:domain rdf:resource="http://example.org/onto/class/google_container_azure_node_pool"/>
    <rdfs:range rdf:resource="http://www.w3.org/2001/XMLSchema#string"/>
  </owl:DatatypeProperty>
  <owl:DatatypeProperty rdf:about="http://example.org/onto/prop/google_container_azure_node_pool_update">
    <rdfs:label>update</rdfs:label>
    <rdfs:domain rdf:resource="http://example.org/onto/class/google_container_azure_node_pool"/>
    <rdfs:range rdf:resource="http://www.w3.org/2001/XMLSchema#string"/>
  </owl:DatatypeProperty>
</rdf:RDF>
