<?xml version="1.0" encoding="UTF-8"?>
<rdf:RDF
  xmlns:rdf="http://www.w3.org/1999/02/22-rdf-syntax-ns#"
  xmlns:rdfs="http://www.w3.org/2000/01/rdf-schema#"
  xmlns:owl="http://www.w3.org/2002/07/owl#"
  xmlns:xsd="http://www.w3.org/2001/XMLSchema#"
  xml:base="http://example.org/onto/">
  <owl:Class rdf:about="http://example.org/onto/class/google_dialogflow_cx_intent">
    <rdfs:label>google_dialogflow_cx_intent</rdfs:label>
    <rdfs:comment>#
#     ***     AUTO GENERATED CODE    ***    Type: MMv1     ***
#
# ----------------------------------------------------------------------------
#
#     This code is generated by Magic Modules using the following:
#
#     Configuration: https:#github.com/GoogleCloudPlatform/magic-modules/tree/main/mmv1/products/dialogflowcx/Intent.yaml
#     Template:      https:#github.com/GoogleCloudPlatform/magic-modules/tree/main/mmv1/templates/terraform/resource.html.markdown.tmpl
#
#     DO NOT EDIT this file directly. Any changes made to this file will be
#     overwritten during the next generation cycle.
#
# ----------------------------------------------------------------------------
subcategory: "Dialogflow CX"
description: |-
  An intent represents a user's intent to interact with a conversational agent.
---</rdfs:comment>
  </owl:Class>
  <owl:DatatypeProperty rdf:about="http://example.org/onto/prop/google_dialogflow_cx_intent_description">
    <rdfs:label>description</rdfs:label>
    <rdfs:comment>Human readable description for better understanding an intent like its scope, content, result etc. Maximum character limit: 140 characters.</rdfs:comment>
    <rdfs:domain rdf:resource="http://example.org/onto/class/google_dialogflow_cx_intent"/>
    <rdfs:range rdf:resource="http://www.w3.org/2001/XMLSchema#string"/>
  </owl:DatatypeProperty>
  <owl:DatatypeProperty rdf:about="http://example.org/onto/prop/google_dialogflow_cx_intent_display_name">
    <rdfs:label>display_name</rdfs:label>
    <rdfs:comment>The human-readable name of the intent, unique within the agent.</rdfs:comment>
    <rdfs:domain rdf:resource="http://example.org/onto/class/google_dialogflow_cx_intent"/>
    <rdfs:range rdf:resource="http://www.w3.org/2001/XMLSchema#string"/>
  </owl:DatatypeProperty>
  <owl:DatatypeProperty rdf:about="http://example.org/onto/prop/google_dialogflow_cx_intent_effective_labels">
    <rdfs:label>effective_labels</rdfs:label>
    <rdfs:comment>All of labels (key/value pairs) present on the resource in GCP, including the labels configured through Terraform, other clients and services.</rdfs:comment>
    <rdfs:domain rdf:resource="http://example.org/onto/class/google_dialogflow_cx_intent"/>
    <rdfs:range rdf:resource="http://www.w3.org/2001/XMLSchema#string"/>
  </owl:DatatypeProperty>
  <owl:DatatypeProperty rdf:about="http://example.org/onto/prop/google_dialogflow_cx_intent_id">
    <rdfs:label>id</rdfs:label>
    <rdfs:domain rdf:resource="http://example.org/onto/class/google_dialogflow_cx_intent"/>
    <rdfs:range rdf:resource="http://www.w3.org/2001/XMLSchema#string"/>
  </owl:DatatypeProperty>
  <owl:DatatypeProperty rdf:about="http://example.org/onto/prop/google_dialogflow_cx_intent_is_default_negative_intent">
    <rdfs:label>is_default_negative_intent</rdfs:label>
    <rdfs:comment>Marks this as the [Default Negative Intent](https://cloud.google.com/dialogflow/cx/docs/concept/intent#negative) for an agent. When you create an agent, a Default Negative Intent is created automatically.
The Default Negative Intent cannot be deleted; deleting the 'google_dialogflow_cx_intent' resource does nothing to the underlying GCP resources.

~> Avoid having multiple 'google_dialogflow_cx_intent' resources linked to the same agent with 'is_default_negative_intent = true' because they will compete to control a single Default Negative Intent resource in GCP.</rdfs:comment>
    <rdfs:domain rdf:resource="http://example.org/onto/class/google_dialogflow_cx_intent"/>
    <rdfs:range rdf:resource="http://www.w3.org/2001/XMLSchema#string"/>
  </owl:DatatypeProperty>
  <owl:DatatypeProperty rdf:about="http://example.org/onto/prop/google_dialogflow_cx_intent_is_default_welcome_intent">
    <rdfs:label>is_default_welcome_intent</rdfs:label>
    <rdfs:comment>Marks this as the [Default Welcome Intent](https://cloud.google.com/dialogflow/cx/docs/concept/intent#welcome) for an agent. When you create an agent, a Default Welcome Intent is created automatically.
The Default Welcome Intent cannot be deleted; deleting the 'google_dialogflow_cx_intent' resource does nothing to the underlying GCP resources.

~> Avoid having multiple 'google_dialogflow_cx_intent' resources linked to the same agent with 'is_default_welcome_intent = true' because they will compete to control a single Default Welcome Intent resource in GCP.</rdfs:comment>
    <rdfs:domain rdf:resource="http://example.org/onto/class/google_dialogflow_cx_intent"/>
    <rdfs:range rdf:resource="http://www.w3.org/2001/XMLSchema#string"/>
  </owl:DatatypeProperty>
  <owl:DatatypeProperty rdf:about="http://example.org/onto/prop/google_dialogflow_cx_intent_is_fallback">
    <rdfs:label>is_fallback</rdfs:label>
    <rdfs:comment>Indicates whether this is a fallback intent. Currently only default fallback intent is allowed in the agent, which is added upon agent creation.
Adding training phrases to fallback intent is useful in the case of requests that are mistakenly matched, since training phrases assigned to fallback intents act as negative examples that triggers no-match event.
To manage the fallback intent, set 'is_default_negative_intent = true'</rdfs:comment>
    <rdfs:domain rdf:resource="http://example.org/onto/class/google_dialogflow_cx_intent"/>
    <rdfs:range rdf:resource="http://www.w3.org/2001/XMLSchema#string"/>
  </owl:DatatypeProperty>
  <owl:DatatypeProperty rdf:about="http://example.org/onto/prop/google_dialogflow_cx_intent_labels">
    <rdfs:label>labels</rdfs:label>
    <rdfs:comment>The key/value metadata to label an intent. Labels can contain lowercase letters, digits and the symbols '-' and '_'. International characters are allowed, including letters from unicase alphabets. Keys must start with a letter. Keys and values can be no longer than 63 characters and no more than 128 bytes.
Prefix "sys-" is reserved for Dialogflow defined labels. Currently allowed Dialogflow defined labels include: * sys-head * sys-contextual The above labels do not require value. "sys-head" means the intent is a head intent. "sys.contextual" means the intent is a contextual intent.
An object containing a list of "key": value pairs. Example: { "name": "wrench", "mass": "1.3kg", "count": "3" }.


**Note**: This field is non-authoritative, and will only manage the labels present in your configuration.
Please refer to the field 'effective_labels' for all of the labels present on the resource.</rdfs:comment>
    <rdfs:domain rdf:resource="http://example.org/onto/class/google_dialogflow_cx_intent"/>
    <rdfs:range rdf:resource="http://www.w3.org/2001/XMLSchema#string"/>
  </owl:DatatypeProperty>
  <owl:DatatypeProperty rdf:about="http://example.org/onto/prop/google_dialogflow_cx_intent_language_code">
    <rdfs:label>language_code</rdfs:label>
    <rdfs:comment>The language of the following fields in intent:
Intent.training_phrases.parts.text
If not specified, the agent's default language is used. Many languages are supported. Note: languages must be enabled in the agent before they can be used.</rdfs:comment>
    <rdfs:domain rdf:resource="http://example.org/onto/class/google_dialogflow_cx_intent"/>
    <rdfs:range rdf:resource="http://www.w3.org/2001/XMLSchema#string"/>
  </owl:DatatypeProperty>
  <owl:DatatypeProperty rdf:about="http://example.org/onto/prop/google_dialogflow_cx_intent_name">
    <rdfs:label>name</rdfs:label>
    <rdfs:comment>The unique identifier of the intent.
Format: projects/<Project ID>/locations/<Location ID>/agents/<Agent ID>/intents/<Intent ID>.</rdfs:comment>
    <rdfs:domain rdf:resource="http://example.org/onto/class/google_dialogflow_cx_intent"/>
    <rdfs:range rdf:resource="http://www.w3.org/2001/XMLSchema#string"/>
  </owl:DatatypeProperty>
  <owl:DatatypeProperty rdf:about="http://example.org/onto/prop/google_dialogflow_cx_intent_parent">
    <rdfs:label>parent</rdfs:label>
    <rdfs:comment>The agent to create an intent for.
Format: projects/<Project ID>/locations/<Location ID>/agents/<Agent ID>.</rdfs:comment>
    <rdfs:domain rdf:resource="http://example.org/onto/class/google_dialogflow_cx_intent"/>
    <rdfs:range rdf:resource="http://www.w3.org/2001/XMLSchema#string"/>
  </owl:DatatypeProperty>
  <owl:DatatypeProperty rdf:about="http://example.org/onto/prop/google_dialogflow_cx_intent_priority">
    <rdfs:label>priority</rdfs:label>
    <rdfs:comment>The priority of this intent. Higher numbers represent higher priorities.
If the supplied value is unspecified or 0, the service translates the value to 500,000, which corresponds to the Normal priority in the console.
If the supplied value is negative, the intent is ignored in runtime detect intent requests.</rdfs:comment>
    <rdfs:domain rdf:resource="http://example.org/onto/class/google_dialogflow_cx_intent"/>
    <rdfs:range rdf:resource="http://www.w3.org/2001/XMLSchema#string"/>
  </owl:DatatypeProperty>
  <owl:DatatypeProperty rdf:about="http://example.org/onto/prop/google_dialogflow_cx_intent_terraform_labels">
    <rdfs:label>terraform_labels</rdfs:label>
    <rdfs:comment>The combination of labels configured directly on the resource
 and default labels configured on the provider.</rdfs:comment>
    <rdfs:domain rdf:resource="http://example.org/onto/class/google_dialogflow_cx_intent"/>
    <rdfs:range rdf:resource="http://www.w3.org/2001/XMLSchema#string"/>
  </owl:DatatypeProperty>
  <owl:DatatypeProperty rdf:about="http://example.org/onto/prop/google_dialogflow_cx_intent_entity_type">
    <rdfs:label>entity_type</rdfs:label>
    <rdfs:comment>The entity type of the parameter.
Format: projects/-/locations/-/agents/-/entityTypes/<System Entity Type ID> for system entity types (for example, projects/-/locations/-/agents/-/entityTypes/sys.date), or projects/<Project ID>/locations/<Location ID>/agents/<Agent ID>/entityTypes/<Entity Type ID> for developer entity types.</rdfs:comment>
    <rdfs:domain rdf:resource="http://example.org/onto/class/google_dialogflow_cx_intent"/>
    <rdfs:range rdf:resource="http://www.w3.org/2001/XMLSchema#string"/>
  </owl:DatatypeProperty>
  <owl:DatatypeProperty rdf:about="http://example.org/onto/prop/google_dialogflow_cx_intent_id">
    <rdfs:label>id</rdfs:label>
    <rdfs:comment>The unique identifier of the parameter. This field is used by training phrases to annotate their parts.</rdfs:comment>
    <rdfs:domain rdf:resource="http://example.org/onto/class/google_dialogflow_cx_intent"/>
    <rdfs:range rdf:resource="http://www.w3.org/2001/XMLSchema#string"/>
  </owl:DatatypeProperty>
  <owl:DatatypeProperty rdf:about="http://example.org/onto/prop/google_dialogflow_cx_intent_is_list">
    <rdfs:label>is_list</rdfs:label>
    <rdfs:comment>Indicates whether the parameter represents a list of values.</rdfs:comment>
    <rdfs:domain rdf:resource="http://example.org/onto/class/google_dialogflow_cx_intent"/>
    <rdfs:range rdf:resource="http://www.w3.org/2001/XMLSchema#string"/>
  </owl:DatatypeProperty>
  <owl:DatatypeProperty rdf:about="http://example.org/onto/prop/google_dialogflow_cx_intent_redact">
    <rdfs:label>redact</rdfs:label>
    <rdfs:comment>Indicates whether the parameter content should be redacted in log. If redaction is enabled, the parameter content will be replaced by parameter name during logging.
Note: the parameter content is subject to redaction if either parameter level redaction or entity type level redaction is enabled.</rdfs:comment>
    <rdfs:domain rdf:resource="http://example.org/onto/class/google_dialogflow_cx_intent"/>
    <rdfs:range rdf:resource="http://www.w3.org/2001/XMLSchema#string"/>
  </owl:DatatypeProperty>
  <owl:DatatypeProperty rdf:about="http://example.org/onto/prop/google_dialogflow_cx_intent_create">
    <rdfs:label>create</rdfs:label>
    <rdfs:domain rdf:resource="http://example.org/onto/class/google_dialogflow_cx_intent"/>
    <rdfs:range rdf:resource="http://www.w3.org/2001/XMLSchema#string"/>
  </owl:DatatypeProperty>
  <owl:DatatypeProperty rdf:about="http://example.org/onto/prop/google_dialogflow_cx_intent_delete">
    <rdfs:label>delete</rdfs:label>
    <rdfs:domain rdf:resource="http://example.org/onto/class/google_dialogflow_cx_intent"/>
    <rdfs:range rdf:resource="http://www.w3.org/2001/XMLSchema#string"/>
  </owl:DatatypeProperty>
  <owl:DatatypeProperty rdf:about="http://example.org/onto/prop/google_dialogflow_cx_intent_update">
    <rdfs:label>update</rdfs:label>
    <rdfs:domain rdf:resource="http://example.org/onto/class/google_dialogflow_cx_intent"/>
    <rdfs:range rdf:resource="http://www.w3.org/2001/XMLSchema#string"/>
  </owl:DatatypeProperty>
  <owl:DatatypeProperty rdf:about="http://example.org/onto/prop/google_dialogflow_cx_intent_id">
    <rdfs:label>id</rdfs:label>
    <rdfs:comment>The unique identifier of the training phrase.</rdfs:comment>
    <rdfs:domain rdf:resource="http://example.org/onto/class/google_dialogflow_cx_intent"/>
    <rdfs:range rdf:resource="http://www.w3.org/2001/XMLSchema#string"/>
  </owl:DatatypeProperty>
  <owl:DatatypeProperty rdf:about="http://example.org/onto/prop/google_dialogflow_cx_intent_repeat_count">
    <rdfs:label>repeat_count</rdfs:label>
    <rdfs:comment>Indicates how many times this example was added to the intent.</rdfs:comment>
    <rdfs:domain rdf:resource="http://example.org/onto/class/google_dialogflow_cx_intent"/>
    <rdfs:range rdf:resource="http://www.w3.org/2001/XMLSchema#string"/>
  </owl:DatatypeProperty>
  <owl:DatatypeProperty rdf:about="http://example.org/onto/prop/google_dialogflow_cx_intent_parameter_id">
    <rdfs:label>parameter_id</rdfs:label>
    <rdfs:comment>The parameter used to annotate this part of the training phrase. This field is required for annotated parts of the training phrase.</rdfs:comment>
    <rdfs:domain rdf:resource="http://example.org/onto/class/google_dialogflow_cx_intent"/>
    <rdfs:range rdf:resource="http://www.w3.org/2001/XMLSchema#string"/>
  </owl:DatatypeProperty>
  <owl:DatatypeProperty rdf:about="http://example.org/onto/prop/google_dialogflow_cx_intent_text">
    <rdfs:label>text</rdfs:label>
    <rdfs:comment>The text for this part.</rdfs:comment>
    <rdfs:domain rdf:resource="http://example.org/onto/class/google_dialogflow_cx_intent"/>
    <rdfs:range rdf:resource="http://www.w3.org/2001/XMLSchema#string"/>
  </owl:DatatypeProperty>
</rdf:RDF>
