<?xml version="1.0" encoding="UTF-8"?>
<rdf:RDF
  xmlns:rdf="http://www.w3.org/1999/02/22-rdf-syntax-ns#"
  xmlns:rdfs="http://www.w3.org/2000/01/rdf-schema#"
  xmlns:owl="http://www.w3.org/2002/07/owl#"
  xmlns:xsd="http://www.w3.org/2001/XMLSchema#"
  xml:base="http://example.org/onto/">
  <owl:Class rdf:about="http://example.org/onto/class/google_compute_route">
    <rdfs:label>google_compute_route</rdfs:label>
    <rdfs:comment>#
#     ***     AUTO GENERATED CODE    ***    Type: MMv1     ***
#
# ----------------------------------------------------------------------------
#
#     This code is generated by Magic Modules using the following:
#
#     Configuration: https:#github.com/GoogleCloudPlatform/magic-modules/tree/main/mmv1/products/compute/Route.yaml
#     Template:      https:#github.com/GoogleCloudPlatform/magic-modules/tree/main/mmv1/templates/terraform/resource.html.markdown.tmpl
#
#     DO NOT EDIT this file directly. Any changes made to this file will be
#     overwritten during the next generation cycle.
#
# ----------------------------------------------------------------------------
subcategory: "Compute Engine"
description: |-
  Represents a Route resource.
---</rdfs:comment>
  </owl:Class>
  <owl:DatatypeProperty rdf:about="http://example.org/onto/prop/google_compute_route_as_paths">
    <rdfs:label>as_paths</rdfs:label>
    <rdfs:domain rdf:resource="http://example.org/onto/class/google_compute_route"/>
    <rdfs:range rdf:resource="http://www.w3.org/2001/XMLSchema#string"/>
  </owl:DatatypeProperty>
  <owl:DatatypeProperty rdf:about="http://example.org/onto/prop/google_compute_route_creation_timestamp">
    <rdfs:label>creation_timestamp</rdfs:label>
    <rdfs:comment>Creation timestamp in RFC3339 text format.</rdfs:comment>
    <rdfs:domain rdf:resource="http://example.org/onto/class/google_compute_route"/>
    <rdfs:range rdf:resource="http://www.w3.org/2001/XMLSchema#string"/>
  </owl:DatatypeProperty>
  <owl:DatatypeProperty rdf:about="http://example.org/onto/prop/google_compute_route_description">
    <rdfs:label>description</rdfs:label>
    <rdfs:comment>An optional description of this resource. Provide this property
when you create the resource.</rdfs:comment>
    <rdfs:domain rdf:resource="http://example.org/onto/class/google_compute_route"/>
    <rdfs:range rdf:resource="http://www.w3.org/2001/XMLSchema#string"/>
  </owl:DatatypeProperty>
  <owl:DatatypeProperty rdf:about="http://example.org/onto/prop/google_compute_route_dest_range">
    <rdfs:label>dest_range</rdfs:label>
    <rdfs:comment>The destination range of outgoing packets that this route applies to.
Only IPv4 is supported.</rdfs:comment>
    <rdfs:domain rdf:resource="http://example.org/onto/class/google_compute_route"/>
    <rdfs:range rdf:resource="http://www.w3.org/2001/XMLSchema#string"/>
  </owl:DatatypeProperty>
  <owl:DatatypeProperty rdf:about="http://example.org/onto/prop/google_compute_route_id">
    <rdfs:label>id</rdfs:label>
    <rdfs:domain rdf:resource="http://example.org/onto/class/google_compute_route"/>
    <rdfs:range rdf:resource="http://www.w3.org/2001/XMLSchema#string"/>
  </owl:DatatypeProperty>
  <owl:DatatypeProperty rdf:about="http://example.org/onto/prop/google_compute_route_name">
    <rdfs:label>name</rdfs:label>
    <rdfs:comment>Name of the resource. Provided by the client when the resource is
created. The name must be 1-63 characters long, and comply with
RFC1035.  Specifically, the name must be 1-63 characters long and
match the regular expression '[a-z]([-a-z0-9]*[a-z0-9])?' which means
the first character must be a lowercase letter, and all following
characters must be a dash, lowercase letter, or digit, except the
last character, which cannot be a dash.</rdfs:comment>
    <rdfs:domain rdf:resource="http://example.org/onto/class/google_compute_route"/>
    <rdfs:range rdf:resource="http://www.w3.org/2001/XMLSchema#string"/>
  </owl:DatatypeProperty>
  <owl:DatatypeProperty rdf:about="http://example.org/onto/prop/google_compute_route_network">
    <rdfs:label>network</rdfs:label>
    <rdfs:comment>The network that this route applies to.</rdfs:comment>
    <rdfs:domain rdf:resource="http://example.org/onto/class/google_compute_route"/>
    <rdfs:range rdf:resource="http://www.w3.org/2001/XMLSchema#string"/>
  </owl:DatatypeProperty>
  <owl:DatatypeProperty rdf:about="http://example.org/onto/prop/google_compute_route_next_hop_gateway">
    <rdfs:label>next_hop_gateway</rdfs:label>
    <rdfs:comment>URL to a gateway that should handle matching packets.
Currently, you can only specify the internet gateway, using a full or
partial valid URL:
* 'https://www.googleapis.com/compute/v1/projects/project/global/gateways/default-internet-gateway'
* 'projects/project/global/gateways/default-internet-gateway'
* 'global/gateways/default-internet-gateway'
* The string 'default-internet-gateway'.</rdfs:comment>
    <rdfs:domain rdf:resource="http://example.org/onto/class/google_compute_route"/>
    <rdfs:range rdf:resource="http://www.w3.org/2001/XMLSchema#string"/>
  </owl:DatatypeProperty>
  <owl:DatatypeProperty rdf:about="http://example.org/onto/prop/google_compute_route_next_hop_hub">
    <rdfs:label>next_hop_hub</rdfs:label>
    <rdfs:comment>The hub network that should handle matching packets, which should conform to RFC1035.</rdfs:comment>
    <rdfs:domain rdf:resource="http://example.org/onto/class/google_compute_route"/>
    <rdfs:range rdf:resource="http://www.w3.org/2001/XMLSchema#string"/>
  </owl:DatatypeProperty>
  <owl:DatatypeProperty rdf:about="http://example.org/onto/prop/google_compute_route_next_hop_ilb">
    <rdfs:label>next_hop_ilb</rdfs:label>
    <rdfs:comment>The IP address or URL to a forwarding rule of type
loadBalancingScheme=INTERNAL that should handle matching
packets.

With the GA provider you can only specify the forwarding
rule as a partial or full URL. For example, the following
are all valid values:
* 10.128.0.56
* https://www.googleapis.com/compute/v1/projects/project/regions/region/forwardingRules/forwardingRule
* regions/region/forwardingRules/forwardingRule

When the beta provider, you can also specify the IP address
of a forwarding rule from the same VPC or any peered VPC.

Note that this can only be used when the destinationRange is
a public (non-RFC 1918) IP CIDR range.</rdfs:comment>
    <rdfs:domain rdf:resource="http://example.org/onto/class/google_compute_route"/>
    <rdfs:range rdf:resource="http://www.w3.org/2001/XMLSchema#string"/>
  </owl:DatatypeProperty>
  <owl:DatatypeProperty rdf:about="http://example.org/onto/prop/google_compute_route_next_hop_instance">
    <rdfs:label>next_hop_instance</rdfs:label>
    <rdfs:comment>URL to an instance that should handle matching packets.
You can specify this as a full or partial URL. For example:
* 'https://www.googleapis.com/compute/v1/projects/project/zones/zone/instances/instance'
* 'projects/project/zones/zone/instances/instance'
* 'zones/zone/instances/instance'
* Just the instance name, with the zone in 'next_hop_instance_zone'.</rdfs:comment>
    <rdfs:domain rdf:resource="http://example.org/onto/class/google_compute_route"/>
    <rdfs:range rdf:resource="http://www.w3.org/2001/XMLSchema#string"/>
  </owl:DatatypeProperty>
  <owl:DatatypeProperty rdf:about="http://example.org/onto/prop/google_compute_route_next_hop_instance_zone">
    <rdfs:label>next_hop_instance_zone</rdfs:label>
    <rdfs:comment>The zone of the instance specified in next_hop_instance. Omit if next_hop_instance is specified as a URL.</rdfs:comment>
    <rdfs:domain rdf:resource="http://example.org/onto/class/google_compute_route"/>
    <rdfs:range rdf:resource="http://www.w3.org/2001/XMLSchema#string"/>
  </owl:DatatypeProperty>
  <owl:DatatypeProperty rdf:about="http://example.org/onto/prop/google_compute_route_next_hop_inter_region_cost">
    <rdfs:label>next_hop_inter_region_cost</rdfs:label>
    <rdfs:comment>Internal fixed region-to-region cost that Google Cloud calculates based on factors such as network performance, distance, and available bandwidth between regions.</rdfs:comment>
    <rdfs:domain rdf:resource="http://example.org/onto/class/google_compute_route"/>
    <rdfs:range rdf:resource="http://www.w3.org/2001/XMLSchema#string"/>
  </owl:DatatypeProperty>
  <owl:DatatypeProperty rdf:about="http://example.org/onto/prop/google_compute_route_next_hop_ip">
    <rdfs:label>next_hop_ip</rdfs:label>
    <rdfs:comment>Network IP address of an instance that should handle matching packets.</rdfs:comment>
    <rdfs:domain rdf:resource="http://example.org/onto/class/google_compute_route"/>
    <rdfs:range rdf:resource="http://www.w3.org/2001/XMLSchema#string"/>
  </owl:DatatypeProperty>
  <owl:DatatypeProperty rdf:about="http://example.org/onto/prop/google_compute_route_next_hop_med">
    <rdfs:label>next_hop_med</rdfs:label>
    <rdfs:comment>Multi-Exit Discriminator, a BGP route metric that indicates the desirability of a particular route in a network.</rdfs:comment>
    <rdfs:domain rdf:resource="http://example.org/onto/class/google_compute_route"/>
    <rdfs:range rdf:resource="http://www.w3.org/2001/XMLSchema#string"/>
  </owl:DatatypeProperty>
  <owl:DatatypeProperty rdf:about="http://example.org/onto/prop/google_compute_route_next_hop_network">
    <rdfs:label>next_hop_network</rdfs:label>
    <rdfs:comment>URL to a Network that should handle matching packets.</rdfs:comment>
    <rdfs:domain rdf:resource="http://example.org/onto/class/google_compute_route"/>
    <rdfs:range rdf:resource="http://www.w3.org/2001/XMLSchema#string"/>
  </owl:DatatypeProperty>
  <owl:DatatypeProperty rdf:about="http://example.org/onto/prop/google_compute_route_next_hop_origin">
    <rdfs:label>next_hop_origin</rdfs:label>
    <rdfs:comment>Indicates the origin of the route. Can be IGP (Interior Gateway Protocol), EGP (Exterior Gateway Protocol), or INCOMPLETE.</rdfs:comment>
    <rdfs:domain rdf:resource="http://example.org/onto/class/google_compute_route"/>
    <rdfs:range rdf:resource="http://www.w3.org/2001/XMLSchema#string"/>
  </owl:DatatypeProperty>
  <owl:DatatypeProperty rdf:about="http://example.org/onto/prop/google_compute_route_next_hop_peering">
    <rdfs:label>next_hop_peering</rdfs:label>
    <rdfs:comment>The network peering name that should handle matching packets, which should conform to RFC1035.</rdfs:comment>
    <rdfs:domain rdf:resource="http://example.org/onto/class/google_compute_route"/>
    <rdfs:range rdf:resource="http://www.w3.org/2001/XMLSchema#string"/>
  </owl:DatatypeProperty>
  <owl:DatatypeProperty rdf:about="http://example.org/onto/prop/google_compute_route_next_hop_vpn_tunnel">
    <rdfs:label>next_hop_vpn_tunnel</rdfs:label>
    <rdfs:comment>URL to a VpnTunnel that should handle matching packets.</rdfs:comment>
    <rdfs:domain rdf:resource="http://example.org/onto/class/google_compute_route"/>
    <rdfs:range rdf:resource="http://www.w3.org/2001/XMLSchema#string"/>
  </owl:DatatypeProperty>
  <owl:DatatypeProperty rdf:about="http://example.org/onto/prop/google_compute_route_priority">
    <rdfs:label>priority</rdfs:label>
    <rdfs:comment>The priority of this route. Priority is used to break ties in cases
where there is more than one matching route of equal prefix length.

In the case of two routes with equal prefix length, the one with the
lowest-numbered priority value wins.

Default value is 1000. Valid range is 0 through 65535.</rdfs:comment>
    <rdfs:domain rdf:resource="http://example.org/onto/class/google_compute_route"/>
    <rdfs:range rdf:resource="http://www.w3.org/2001/XMLSchema#string"/>
  </owl:DatatypeProperty>
  <owl:DatatypeProperty rdf:about="http://example.org/onto/prop/google_compute_route_project">
    <rdfs:label>project</rdfs:label>
    <rdfs:domain rdf:resource="http://example.org/onto/class/google_compute_route"/>
    <rdfs:range rdf:resource="http://www.w3.org/2001/XMLSchema#string"/>
  </owl:DatatypeProperty>
  <owl:DatatypeProperty rdf:about="http://example.org/onto/prop/google_compute_route_route_status">
    <rdfs:label>route_status</rdfs:label>
    <rdfs:comment>The status of the route, which can be one of the following values:
- 'ACTIVE' for an active route
- 'INACTIVE' for an inactive route</rdfs:comment>
    <rdfs:domain rdf:resource="http://example.org/onto/class/google_compute_route"/>
    <rdfs:range rdf:resource="http://www.w3.org/2001/XMLSchema#string"/>
  </owl:DatatypeProperty>
  <owl:DatatypeProperty rdf:about="http://example.org/onto/prop/google_compute_route_route_type">
    <rdfs:label>route_type</rdfs:label>
    <rdfs:comment>The type of this route, which can be one of the following values:
- 'TRANSIT' for a transit route that this router learned from another Cloud Router and will readvertise to one of its BGP peers
- 'SUBNET' for a route from a subnet of the VPC
- 'BGP' for a route learned from a BGP peer of this router
- 'STATIC' for a static route</rdfs:comment>
    <rdfs:domain rdf:resource="http://example.org/onto/class/google_compute_route"/>
    <rdfs:range rdf:resource="http://www.w3.org/2001/XMLSchema#string"/>
  </owl:DatatypeProperty>
  <owl:DatatypeProperty rdf:about="http://example.org/onto/prop/google_compute_route_self_link">
    <rdfs:label>self_link</rdfs:label>
    <rdfs:domain rdf:resource="http://example.org/onto/class/google_compute_route"/>
    <rdfs:range rdf:resource="http://www.w3.org/2001/XMLSchema#string"/>
  </owl:DatatypeProperty>
  <owl:DatatypeProperty rdf:about="http://example.org/onto/prop/google_compute_route_tags">
    <rdfs:label>tags</rdfs:label>
    <rdfs:comment>A list of instance tags to which this route applies.</rdfs:comment>
    <rdfs:domain rdf:resource="http://example.org/onto/class/google_compute_route"/>
    <rdfs:range rdf:resource="http://www.w3.org/2001/XMLSchema#string"/>
  </owl:DatatypeProperty>
  <owl:DatatypeProperty rdf:about="http://example.org/onto/prop/google_compute_route_warnings">
    <rdfs:label>warnings</rdfs:label>
    <rdfs:comment>If potential misconfigurations are detected for this route, this field will be populated with warning messages.</rdfs:comment>
    <rdfs:domain rdf:resource="http://example.org/onto/class/google_compute_route"/>
    <rdfs:range rdf:resource="http://www.w3.org/2001/XMLSchema#string"/>
  </owl:DatatypeProperty>
  <owl:DatatypeProperty rdf:about="http://example.org/onto/prop/google_compute_route_resource_manager_tags">
    <rdfs:label>resource_manager_tags</rdfs:label>
    <rdfs:comment>Resource manager tags to be bound to the route. Tag keys and values have the
same definition as resource manager tags. Keys must be in the format tagKeys/{tag_key_id},
and values are in the format tagValues/456. The field is ignored when empty.
The field is immutable and causes resource replacement when mutated. This field is only
set at create time and modifying this field after creation will trigger recreation.
To apply tags to an existing resource, see the google_tags_tag_binding resource.</rdfs:comment>
    <rdfs:domain rdf:resource="http://example.org/onto/class/google_compute_route"/>
    <rdfs:range rdf:resource="http://www.w3.org/2001/XMLSchema#string"/>
  </owl:DatatypeProperty>
  <owl:DatatypeProperty rdf:about="http://example.org/onto/prop/google_compute_route_create">
    <rdfs:label>create</rdfs:label>
    <rdfs:domain rdf:resource="http://example.org/onto/class/google_compute_route"/>
    <rdfs:range rdf:resource="http://www.w3.org/2001/XMLSchema#string"/>
  </owl:DatatypeProperty>
  <owl:DatatypeProperty rdf:about="http://example.org/onto/prop/google_compute_route_delete">
    <rdfs:label>delete</rdfs:label>
    <rdfs:domain rdf:resource="http://example.org/onto/class/google_compute_route"/>
    <rdfs:range rdf:resource="http://www.w3.org/2001/XMLSchema#string"/>
  </owl:DatatypeProperty>
</rdf:RDF>
