<?xml version="1.0" encoding="UTF-8"?>
<rdf:RDF
  xmlns:rdf="http://www.w3.org/1999/02/22-rdf-syntax-ns#"
  xmlns:rdfs="http://www.w3.org/2000/01/rdf-schema#"
  xmlns:owl="http://www.w3.org/2002/07/owl#"
  xmlns:xsd="http://www.w3.org/2001/XMLSchema#"
  xml:base="http://example.org/onto/">
  <owl:Class rdf:about="http://example.org/onto/class/google_kms_secret_ciphertext">
    <rdfs:label>google_kms_secret_ciphertext</rdfs:label>
    <rdfs:comment>#
#     ***     AUTO GENERATED CODE    ***    Type: MMv1     ***
#
# ----------------------------------------------------------------------------
#
#     This code is generated by Magic Modules using the following:
#
#     Configuration: https:#github.com/GoogleCloudPlatform/magic-modules/tree/main/mmv1/products/kms/SecretCiphertext.yaml
#     Template:      https:#github.com/GoogleCloudPlatform/magic-modules/tree/main/mmv1/templates/terraform/resource.html.markdown.tmpl
#
#     DO NOT EDIT this file directly. Any changes made to this file will be
#     overwritten during the next generation cycle.
#
# ----------------------------------------------------------------------------
subcategory: "Cloud Key Management Service"
description: |-
  Encrypts secret data with Google Cloud KMS and provides access to the ciphertext.
---</rdfs:comment>
  </owl:Class>
  <owl:DatatypeProperty rdf:about="http://example.org/onto/prop/google_kms_secret_ciphertext_additional_authenticated_data">
    <rdfs:label>additional_authenticated_data</rdfs:label>
    <rdfs:comment>The additional authenticated data used for integrity checks during encryption and decryption.</rdfs:comment>
    <rdfs:domain rdf:resource="http://example.org/onto/class/google_kms_secret_ciphertext"/>
    <rdfs:range rdf:resource="http://www.w3.org/2001/XMLSchema#string"/>
  </owl:DatatypeProperty>
  <owl:DatatypeProperty rdf:about="http://example.org/onto/prop/google_kms_secret_ciphertext_ciphertext">
    <rdfs:label>ciphertext</rdfs:label>
    <rdfs:comment>Contains the result of encrypting the provided plaintext, encoded in base64.</rdfs:comment>
    <rdfs:domain rdf:resource="http://example.org/onto/class/google_kms_secret_ciphertext"/>
    <rdfs:range rdf:resource="http://www.w3.org/2001/XMLSchema#string"/>
  </owl:DatatypeProperty>
  <owl:DatatypeProperty rdf:about="http://example.org/onto/prop/google_kms_secret_ciphertext_crypto_key">
    <rdfs:label>crypto_key</rdfs:label>
    <rdfs:comment>The full name of the CryptoKey that will be used to encrypt the provided plaintext.
Format: ''projects/{{project}}/locations/{{location}}/keyRings/{{keyRing}}/cryptoKeys/{{cryptoKey}}''</rdfs:comment>
    <rdfs:domain rdf:resource="http://example.org/onto/class/google_kms_secret_ciphertext"/>
    <rdfs:range rdf:resource="http://www.w3.org/2001/XMLSchema#string"/>
  </owl:DatatypeProperty>
  <owl:DatatypeProperty rdf:about="http://example.org/onto/prop/google_kms_secret_ciphertext_id">
    <rdfs:label>id</rdfs:label>
    <rdfs:domain rdf:resource="http://example.org/onto/class/google_kms_secret_ciphertext"/>
    <rdfs:range rdf:resource="http://www.w3.org/2001/XMLSchema#string"/>
  </owl:DatatypeProperty>
  <owl:DatatypeProperty rdf:about="http://example.org/onto/prop/google_kms_secret_ciphertext_plaintext">
    <rdfs:label>plaintext</rdfs:label>
    <rdfs:comment>The plaintext to be encrypted.</rdfs:comment>
    <rdfs:domain rdf:resource="http://example.org/onto/class/google_kms_secret_ciphertext"/>
    <rdfs:range rdf:resource="http://www.w3.org/2001/XMLSchema#string"/>
  </owl:DatatypeProperty>
  <owl:DatatypeProperty rdf:about="http://example.org/onto/prop/google_kms_secret_ciphertext_create">
    <rdfs:label>create</rdfs:label>
    <rdfs:domain rdf:resource="http://example.org/onto/class/google_kms_secret_ciphertext"/>
    <rdfs:range rdf:resource="http://www.w3.org/2001/XMLSchema#string"/>
  </owl:DatatypeProperty>
  <owl:DatatypeProperty rdf:about="http://example.org/onto/prop/google_kms_secret_ciphertext_delete">
    <rdfs:label>delete</rdfs:label>
    <rdfs:domain rdf:resource="http://example.org/onto/class/google_kms_secret_ciphertext"/>
    <rdfs:range rdf:resource="http://www.w3.org/2001/XMLSchema#string"/>
  </owl:DatatypeProperty>
</rdf:RDF>
