<?xml version="1.0" encoding="UTF-8"?>
<rdf:RDF
  xmlns:rdf="http://www.w3.org/1999/02/22-rdf-syntax-ns#"
  xmlns:rdfs="http://www.w3.org/2000/01/rdf-schema#"
  xmlns:owl="http://www.w3.org/2002/07/owl#"
  xmlns:xsd="http://www.w3.org/2001/XMLSchema#"
  xml:base="http://example.org/onto/">
  <owl:Class rdf:about="http://example.org/onto/class/google_apigee_target_server">
    <rdfs:label>google_apigee_target_server</rdfs:label>
    <rdfs:comment>#
#     ***     AUTO GENERATED CODE    ***    Type: MMv1     ***
#
# ----------------------------------------------------------------------------
#
#     This code is generated by Magic Modules using the following:
#
#     Configuration: https:#github.com/GoogleCloudPlatform/magic-modules/tree/main/mmv1/products/apigee/TargetServer.yaml
#     Template:      https:#github.com/GoogleCloudPlatform/magic-modules/tree/main/mmv1/templates/terraform/resource.html.markdown.tmpl
#
#     DO NOT EDIT this file directly. Any changes made to this file will be
#     overwritten during the next generation cycle.
#
# ----------------------------------------------------------------------------
subcategory: "Apigee"
description: |-
  TargetServer configuration.
---</rdfs:comment>
  </owl:Class>
  <owl:DatatypeProperty rdf:about="http://example.org/onto/prop/google_apigee_target_server_description">
    <rdfs:label>description</rdfs:label>
    <rdfs:comment>A human-readable description of this TargetServer.</rdfs:comment>
    <rdfs:domain rdf:resource="http://example.org/onto/class/google_apigee_target_server"/>
    <rdfs:range rdf:resource="http://www.w3.org/2001/XMLSchema#string"/>
  </owl:DatatypeProperty>
  <owl:DatatypeProperty rdf:about="http://example.org/onto/prop/google_apigee_target_server_env_id">
    <rdfs:label>env_id</rdfs:label>
    <rdfs:comment>The Apigee environment group associated with the Apigee environment,
in the format 'organizations/{{org_name}}/environments/{{env_name}}'.</rdfs:comment>
    <rdfs:domain rdf:resource="http://example.org/onto/class/google_apigee_target_server"/>
    <rdfs:range rdf:resource="http://www.w3.org/2001/XMLSchema#string"/>
  </owl:DatatypeProperty>
  <owl:DatatypeProperty rdf:about="http://example.org/onto/prop/google_apigee_target_server_host">
    <rdfs:label>host</rdfs:label>
    <rdfs:comment>The host name this target connects to. Value must be a valid hostname as described by RFC-1123.</rdfs:comment>
    <rdfs:domain rdf:resource="http://example.org/onto/class/google_apigee_target_server"/>
    <rdfs:range rdf:resource="http://www.w3.org/2001/XMLSchema#string"/>
  </owl:DatatypeProperty>
  <owl:DatatypeProperty rdf:about="http://example.org/onto/prop/google_apigee_target_server_id">
    <rdfs:label>id</rdfs:label>
    <rdfs:domain rdf:resource="http://example.org/onto/class/google_apigee_target_server"/>
    <rdfs:range rdf:resource="http://www.w3.org/2001/XMLSchema#string"/>
  </owl:DatatypeProperty>
  <owl:DatatypeProperty rdf:about="http://example.org/onto/prop/google_apigee_target_server_is_enabled">
    <rdfs:label>is_enabled</rdfs:label>
    <rdfs:comment>Enabling/disabling a TargetServer is useful when TargetServers are used in load balancing configurations, and one or more TargetServers need to taken out of rotation periodically. Defaults to true.</rdfs:comment>
    <rdfs:domain rdf:resource="http://example.org/onto/class/google_apigee_target_server"/>
    <rdfs:range rdf:resource="http://www.w3.org/2001/XMLSchema#string"/>
  </owl:DatatypeProperty>
  <owl:DatatypeProperty rdf:about="http://example.org/onto/prop/google_apigee_target_server_name">
    <rdfs:label>name</rdfs:label>
    <rdfs:comment>The resource id of this reference. Values must match the regular expression [\w\s-.]+.</rdfs:comment>
    <rdfs:domain rdf:resource="http://example.org/onto/class/google_apigee_target_server"/>
    <rdfs:range rdf:resource="http://www.w3.org/2001/XMLSchema#string"/>
  </owl:DatatypeProperty>
  <owl:DatatypeProperty rdf:about="http://example.org/onto/prop/google_apigee_target_server_port">
    <rdfs:label>port</rdfs:label>
    <rdfs:comment>The port number this target connects to on the given host. Value must be between 1 and 65535, inclusive.</rdfs:comment>
    <rdfs:domain rdf:resource="http://example.org/onto/class/google_apigee_target_server"/>
    <rdfs:range rdf:resource="http://www.w3.org/2001/XMLSchema#string"/>
  </owl:DatatypeProperty>
  <owl:DatatypeProperty rdf:about="http://example.org/onto/prop/google_apigee_target_server_protocol">
    <rdfs:label>protocol</rdfs:label>
    <rdfs:comment>Immutable. The protocol used by this TargetServer. Possible values: ["HTTP", "HTTP2", "GRPC_TARGET", "GRPC", "EXTERNAL_CALLOUT"]</rdfs:comment>
    <rdfs:domain rdf:resource="http://example.org/onto/class/google_apigee_target_server"/>
    <rdfs:range rdf:resource="http://www.w3.org/2001/XMLSchema#string"/>
  </owl:DatatypeProperty>
  <owl:DatatypeProperty rdf:about="http://example.org/onto/prop/google_apigee_target_server_ciphers">
    <rdfs:label>ciphers</rdfs:label>
    <rdfs:comment>The SSL/TLS cipher suites to be used. For programmable proxies, it must be one of the cipher suite names listed in: http://docs.oracle.com/javase/8/docs/technotes/guides/security/StandardNames.html#ciphersuites. For configurable proxies, it must follow the configuration specified in: https://commondatastorage.googleapis.com/chromium-boringssl-docs/ssl.h.html#Cipher-suite-configuration. This setting has no effect for configurable proxies when negotiating TLS 1.3.</rdfs:comment>
    <rdfs:domain rdf:resource="http://example.org/onto/class/google_apigee_target_server"/>
    <rdfs:range rdf:resource="http://www.w3.org/2001/XMLSchema#string"/>
  </owl:DatatypeProperty>
  <owl:DatatypeProperty rdf:about="http://example.org/onto/prop/google_apigee_target_server_client_auth_enabled">
    <rdfs:label>client_auth_enabled</rdfs:label>
    <rdfs:comment>Enables two-way TLS.</rdfs:comment>
    <rdfs:domain rdf:resource="http://example.org/onto/class/google_apigee_target_server"/>
    <rdfs:range rdf:resource="http://www.w3.org/2001/XMLSchema#string"/>
  </owl:DatatypeProperty>
  <owl:DatatypeProperty rdf:about="http://example.org/onto/prop/google_apigee_target_server_enabled">
    <rdfs:label>enabled</rdfs:label>
    <rdfs:comment>Enables TLS. If false, neither one-way nor two-way TLS will be enabled.</rdfs:comment>
    <rdfs:domain rdf:resource="http://example.org/onto/class/google_apigee_target_server"/>
    <rdfs:range rdf:resource="http://www.w3.org/2001/XMLSchema#string"/>
  </owl:DatatypeProperty>
  <owl:DatatypeProperty rdf:about="http://example.org/onto/prop/google_apigee_target_server_enforce">
    <rdfs:label>enforce</rdfs:label>
    <rdfs:comment>If true, TLS is strictly enforced.</rdfs:comment>
    <rdfs:domain rdf:resource="http://example.org/onto/class/google_apigee_target_server"/>
    <rdfs:range rdf:resource="http://www.w3.org/2001/XMLSchema#string"/>
  </owl:DatatypeProperty>
  <owl:DatatypeProperty rdf:about="http://example.org/onto/prop/google_apigee_target_server_ignore_validation_errors">
    <rdfs:label>ignore_validation_errors</rdfs:label>
    <rdfs:comment>If true, Edge ignores TLS certificate errors. Valid when configuring TLS for target servers and target endpoints, and when configuring virtual hosts that use 2-way TLS. When used with a target endpoint/target server, if the backend system uses SNI and returns a cert with a subject Distinguished Name (DN) that does not match the hostname, there is no way to ignore the error and the connection fails.</rdfs:comment>
    <rdfs:domain rdf:resource="http://example.org/onto/class/google_apigee_target_server"/>
    <rdfs:range rdf:resource="http://www.w3.org/2001/XMLSchema#string"/>
  </owl:DatatypeProperty>
  <owl:DatatypeProperty rdf:about="http://example.org/onto/prop/google_apigee_target_server_key_alias">
    <rdfs:label>key_alias</rdfs:label>
    <rdfs:comment>Required if clientAuthEnabled is true. The resource ID for the alias containing the private key and cert.</rdfs:comment>
    <rdfs:domain rdf:resource="http://example.org/onto/class/google_apigee_target_server"/>
    <rdfs:range rdf:resource="http://www.w3.org/2001/XMLSchema#string"/>
  </owl:DatatypeProperty>
  <owl:DatatypeProperty rdf:about="http://example.org/onto/prop/google_apigee_target_server_key_store">
    <rdfs:label>key_store</rdfs:label>
    <rdfs:comment>Required if clientAuthEnabled is true. The resource ID of the keystore.</rdfs:comment>
    <rdfs:domain rdf:resource="http://example.org/onto/class/google_apigee_target_server"/>
    <rdfs:range rdf:resource="http://www.w3.org/2001/XMLSchema#string"/>
  </owl:DatatypeProperty>
  <owl:DatatypeProperty rdf:about="http://example.org/onto/prop/google_apigee_target_server_protocols">
    <rdfs:label>protocols</rdfs:label>
    <rdfs:comment>The TLS versioins to be used.</rdfs:comment>
    <rdfs:domain rdf:resource="http://example.org/onto/class/google_apigee_target_server"/>
    <rdfs:range rdf:resource="http://www.w3.org/2001/XMLSchema#string"/>
  </owl:DatatypeProperty>
  <owl:DatatypeProperty rdf:about="http://example.org/onto/prop/google_apigee_target_server_trust_store">
    <rdfs:label>trust_store</rdfs:label>
    <rdfs:comment>The resource ID of the truststore.</rdfs:comment>
    <rdfs:domain rdf:resource="http://example.org/onto/class/google_apigee_target_server"/>
    <rdfs:range rdf:resource="http://www.w3.org/2001/XMLSchema#string"/>
  </owl:DatatypeProperty>
  <owl:DatatypeProperty rdf:about="http://example.org/onto/prop/google_apigee_target_server_value">
    <rdfs:label>value</rdfs:label>
    <rdfs:comment>The TLS Common Name string of the certificate.</rdfs:comment>
    <rdfs:domain rdf:resource="http://example.org/onto/class/google_apigee_target_server"/>
    <rdfs:range rdf:resource="http://www.w3.org/2001/XMLSchema#string"/>
  </owl:DatatypeProperty>
  <owl:DatatypeProperty rdf:about="http://example.org/onto/prop/google_apigee_target_server_wildcard_match">
    <rdfs:label>wildcard_match</rdfs:label>
    <rdfs:comment>Indicates whether the cert should be matched against as a wildcard cert.</rdfs:comment>
    <rdfs:domain rdf:resource="http://example.org/onto/class/google_apigee_target_server"/>
    <rdfs:range rdf:resource="http://www.w3.org/2001/XMLSchema#string"/>
  </owl:DatatypeProperty>
  <owl:DatatypeProperty rdf:about="http://example.org/onto/prop/google_apigee_target_server_create">
    <rdfs:label>create</rdfs:label>
    <rdfs:domain rdf:resource="http://example.org/onto/class/google_apigee_target_server"/>
    <rdfs:range rdf:resource="http://www.w3.org/2001/XMLSchema#string"/>
  </owl:DatatypeProperty>
  <owl:DatatypeProperty rdf:about="http://example.org/onto/prop/google_apigee_target_server_delete">
    <rdfs:label>delete</rdfs:label>
    <rdfs:domain rdf:resource="http://example.org/onto/class/google_apigee_target_server"/>
    <rdfs:range rdf:resource="http://www.w3.org/2001/XMLSchema#string"/>
  </owl:DatatypeProperty>
  <owl:DatatypeProperty rdf:about="http://example.org/onto/prop/google_apigee_target_server_update">
    <rdfs:label>update</rdfs:label>
    <rdfs:domain rdf:resource="http://example.org/onto/class/google_apigee_target_server"/>
    <rdfs:range rdf:resource="http://www.w3.org/2001/XMLSchema#string"/>
  </owl:DatatypeProperty>
</rdf:RDF>
