<?xml version="1.0" encoding="UTF-8"?>
<rdf:RDF
  xmlns:rdf="http://www.w3.org/1999/02/22-rdf-syntax-ns#"
  xmlns:rdfs="http://www.w3.org/2000/01/rdf-schema#"
  xmlns:owl="http://www.w3.org/2002/07/owl#"
  xmlns:xsd="http://www.w3.org/2001/XMLSchema#"
  xml:base="http://example.org/onto/">
  <owl:Class rdf:about="http://example.org/onto/class/google_compute_image">
    <rdfs:label>google_compute_image</rdfs:label>
    <rdfs:comment>#
#     ***     AUTO GENERATED CODE    ***    Type: MMv1     ***
#
# ----------------------------------------------------------------------------
#
#     This code is generated by Magic Modules using the following:
#
#     Configuration: https:#github.com/GoogleCloudPlatform/magic-modules/tree/main/mmv1/products/compute/Image.yaml
#     Template:      https:#github.com/GoogleCloudPlatform/magic-modules/tree/main/mmv1/templates/terraform/resource.html.markdown.tmpl
#
#     DO NOT EDIT this file directly. Any changes made to this file will be
#     overwritten during the next generation cycle.
#
# ----------------------------------------------------------------------------
subcategory: "Compute Engine"
description: |-
  Represents an Image resource.
---</rdfs:comment>
  </owl:Class>
  <owl:DatatypeProperty rdf:about="http://example.org/onto/prop/google_compute_image_archive_size_bytes">
    <rdfs:label>archive_size_bytes</rdfs:label>
    <rdfs:comment>Size of the image tar.gz archive stored in Google Cloud Storage (in
bytes).</rdfs:comment>
    <rdfs:domain rdf:resource="http://example.org/onto/class/google_compute_image"/>
    <rdfs:range rdf:resource="http://www.w3.org/2001/XMLSchema#string"/>
  </owl:DatatypeProperty>
  <owl:DatatypeProperty rdf:about="http://example.org/onto/prop/google_compute_image_creation_timestamp">
    <rdfs:label>creation_timestamp</rdfs:label>
    <rdfs:comment>Creation timestamp in RFC3339 text format.</rdfs:comment>
    <rdfs:domain rdf:resource="http://example.org/onto/class/google_compute_image"/>
    <rdfs:range rdf:resource="http://www.w3.org/2001/XMLSchema#string"/>
  </owl:DatatypeProperty>
  <owl:DatatypeProperty rdf:about="http://example.org/onto/prop/google_compute_image_description">
    <rdfs:label>description</rdfs:label>
    <rdfs:comment>An optional description of this resource. Provide this property when
you create the resource.</rdfs:comment>
    <rdfs:domain rdf:resource="http://example.org/onto/class/google_compute_image"/>
    <rdfs:range rdf:resource="http://www.w3.org/2001/XMLSchema#string"/>
  </owl:DatatypeProperty>
  <owl:DatatypeProperty rdf:about="http://example.org/onto/prop/google_compute_image_disk_size_gb">
    <rdfs:label>disk_size_gb</rdfs:label>
    <rdfs:comment>Size of the image when restored onto a persistent disk (in GB).</rdfs:comment>
    <rdfs:domain rdf:resource="http://example.org/onto/class/google_compute_image"/>
    <rdfs:range rdf:resource="http://www.w3.org/2001/XMLSchema#string"/>
  </owl:DatatypeProperty>
  <owl:DatatypeProperty rdf:about="http://example.org/onto/prop/google_compute_image_effective_labels">
    <rdfs:label>effective_labels</rdfs:label>
    <rdfs:comment>All of labels (key/value pairs) present on the resource in GCP, including the labels configured through Terraform, other clients and services.</rdfs:comment>
    <rdfs:domain rdf:resource="http://example.org/onto/class/google_compute_image"/>
    <rdfs:range rdf:resource="http://www.w3.org/2001/XMLSchema#string"/>
  </owl:DatatypeProperty>
  <owl:DatatypeProperty rdf:about="http://example.org/onto/prop/google_compute_image_family">
    <rdfs:label>family</rdfs:label>
    <rdfs:comment>The name of the image family to which this image belongs. You can
create disks by specifying an image family instead of a specific
image name. The image family always returns its latest image that is
not deprecated. The name of the image family must comply with
RFC1035.</rdfs:comment>
    <rdfs:domain rdf:resource="http://example.org/onto/class/google_compute_image"/>
    <rdfs:range rdf:resource="http://www.w3.org/2001/XMLSchema#string"/>
  </owl:DatatypeProperty>
  <owl:DatatypeProperty rdf:about="http://example.org/onto/prop/google_compute_image_id">
    <rdfs:label>id</rdfs:label>
    <rdfs:domain rdf:resource="http://example.org/onto/class/google_compute_image"/>
    <rdfs:range rdf:resource="http://www.w3.org/2001/XMLSchema#string"/>
  </owl:DatatypeProperty>
  <owl:DatatypeProperty rdf:about="http://example.org/onto/prop/google_compute_image_label_fingerprint">
    <rdfs:label>label_fingerprint</rdfs:label>
    <rdfs:comment>The fingerprint used for optimistic locking of this resource. Used
internally during updates.</rdfs:comment>
    <rdfs:domain rdf:resource="http://example.org/onto/class/google_compute_image"/>
    <rdfs:range rdf:resource="http://www.w3.org/2001/XMLSchema#string"/>
  </owl:DatatypeProperty>
  <owl:DatatypeProperty rdf:about="http://example.org/onto/prop/google_compute_image_labels">
    <rdfs:label>labels</rdfs:label>
    <rdfs:comment>Labels to apply to this Image.

**Note**: This field is non-authoritative, and will only manage the labels present in your configuration.
Please refer to the field 'effective_labels' for all of the labels present on the resource.</rdfs:comment>
    <rdfs:domain rdf:resource="http://example.org/onto/class/google_compute_image"/>
    <rdfs:range rdf:resource="http://www.w3.org/2001/XMLSchema#string"/>
  </owl:DatatypeProperty>
  <owl:DatatypeProperty rdf:about="http://example.org/onto/prop/google_compute_image_licenses">
    <rdfs:label>licenses</rdfs:label>
    <rdfs:comment>Any applicable license URI.</rdfs:comment>
    <rdfs:domain rdf:resource="http://example.org/onto/class/google_compute_image"/>
    <rdfs:range rdf:resource="http://www.w3.org/2001/XMLSchema#string"/>
  </owl:DatatypeProperty>
  <owl:DatatypeProperty rdf:about="http://example.org/onto/prop/google_compute_image_name">
    <rdfs:label>name</rdfs:label>
    <rdfs:comment>Name of the resource; provided by the client when the resource is
created. The name must be 1-63 characters long, and comply with
RFC1035. Specifically, the name must be 1-63 characters long and
match the regular expression '[a-z]([-a-z0-9]*[a-z0-9])?' which means
the first character must be a lowercase letter, and all following
characters must be a dash, lowercase letter, or digit, except the
last character, which cannot be a dash.</rdfs:comment>
    <rdfs:domain rdf:resource="http://example.org/onto/class/google_compute_image"/>
    <rdfs:range rdf:resource="http://www.w3.org/2001/XMLSchema#string"/>
  </owl:DatatypeProperty>
  <owl:DatatypeProperty rdf:about="http://example.org/onto/prop/google_compute_image_project">
    <rdfs:label>project</rdfs:label>
    <rdfs:domain rdf:resource="http://example.org/onto/class/google_compute_image"/>
    <rdfs:range rdf:resource="http://www.w3.org/2001/XMLSchema#string"/>
  </owl:DatatypeProperty>
  <owl:DatatypeProperty rdf:about="http://example.org/onto/prop/google_compute_image_self_link">
    <rdfs:label>self_link</rdfs:label>
    <rdfs:domain rdf:resource="http://example.org/onto/class/google_compute_image"/>
    <rdfs:range rdf:resource="http://www.w3.org/2001/XMLSchema#string"/>
  </owl:DatatypeProperty>
  <owl:DatatypeProperty rdf:about="http://example.org/onto/prop/google_compute_image_source_disk">
    <rdfs:label>source_disk</rdfs:label>
    <rdfs:comment>The source disk to create this image based on.
You must provide either this property or the
rawDisk.source property but not both to create an image.</rdfs:comment>
    <rdfs:domain rdf:resource="http://example.org/onto/class/google_compute_image"/>
    <rdfs:range rdf:resource="http://www.w3.org/2001/XMLSchema#string"/>
  </owl:DatatypeProperty>
  <owl:DatatypeProperty rdf:about="http://example.org/onto/prop/google_compute_image_source_image">
    <rdfs:label>source_image</rdfs:label>
    <rdfs:comment>URL of the source image used to create this image. In order to create an image, you must provide the full or partial
URL of one of the following:

* The selfLink URL
* This property
* The rawDisk.source URL
* The sourceDisk URL</rdfs:comment>
    <rdfs:domain rdf:resource="http://example.org/onto/class/google_compute_image"/>
    <rdfs:range rdf:resource="http://www.w3.org/2001/XMLSchema#string"/>
  </owl:DatatypeProperty>
  <owl:DatatypeProperty rdf:about="http://example.org/onto/prop/google_compute_image_source_snapshot">
    <rdfs:label>source_snapshot</rdfs:label>
    <rdfs:comment>URL of the source snapshot used to create this image.

In order to create an image, you must provide the full or partial URL of one of the following:

* The selfLink URL
* This property
* The sourceImage URL
* The rawDisk.source URL
* The sourceDisk URL</rdfs:comment>
    <rdfs:domain rdf:resource="http://example.org/onto/class/google_compute_image"/>
    <rdfs:range rdf:resource="http://www.w3.org/2001/XMLSchema#string"/>
  </owl:DatatypeProperty>
  <owl:DatatypeProperty rdf:about="http://example.org/onto/prop/google_compute_image_storage_locations">
    <rdfs:label>storage_locations</rdfs:label>
    <rdfs:comment>Cloud Storage bucket storage location of the image
(regional or multi-regional).
Reference link: https://cloud.google.com/compute/docs/reference/rest/v1/images</rdfs:comment>
    <rdfs:domain rdf:resource="http://example.org/onto/class/google_compute_image"/>
    <rdfs:range rdf:resource="http://www.w3.org/2001/XMLSchema#string"/>
  </owl:DatatypeProperty>
  <owl:DatatypeProperty rdf:about="http://example.org/onto/prop/google_compute_image_terraform_labels">
    <rdfs:label>terraform_labels</rdfs:label>
    <rdfs:comment>The combination of labels configured directly on the resource
 and default labels configured on the provider.</rdfs:comment>
    <rdfs:domain rdf:resource="http://example.org/onto/class/google_compute_image"/>
    <rdfs:range rdf:resource="http://www.w3.org/2001/XMLSchema#string"/>
  </owl:DatatypeProperty>
  <owl:DatatypeProperty rdf:about="http://example.org/onto/prop/google_compute_image_type">
    <rdfs:label>type</rdfs:label>
    <rdfs:comment>The type of supported feature. Read [Enabling guest operating system features](https://cloud.google.com/compute/docs/images/create-delete-deprecate-private-images#guest-os-features) to see a list of available options. Possible values: ["MULTI_IP_SUBNET", "SECURE_BOOT", "SEV_CAPABLE", "UEFI_COMPATIBLE", "VIRTIO_SCSI_MULTIQUEUE", "WINDOWS", "GVNIC", "IDPF", "SEV_LIVE_MIGRATABLE", "SEV_SNP_CAPABLE", "SUSPEND_RESUME_COMPATIBLE", "TDX_CAPABLE", "SEV_LIVE_MIGRATABLE_V2"]</rdfs:comment>
    <rdfs:domain rdf:resource="http://example.org/onto/class/google_compute_image"/>
    <rdfs:range rdf:resource="http://www.w3.org/2001/XMLSchema#string"/>
  </owl:DatatypeProperty>
  <owl:DatatypeProperty rdf:about="http://example.org/onto/prop/google_compute_image_kms_key_self_link">
    <rdfs:label>kms_key_self_link</rdfs:label>
    <rdfs:comment>The self link of the encryption key that is stored in Google Cloud
KMS.</rdfs:comment>
    <rdfs:domain rdf:resource="http://example.org/onto/class/google_compute_image"/>
    <rdfs:range rdf:resource="http://www.w3.org/2001/XMLSchema#string"/>
  </owl:DatatypeProperty>
  <owl:DatatypeProperty rdf:about="http://example.org/onto/prop/google_compute_image_kms_key_service_account">
    <rdfs:label>kms_key_service_account</rdfs:label>
    <rdfs:comment>The service account being used for the encryption request for the
given KMS key. If absent, the Compute Engine default service
account is used.</rdfs:comment>
    <rdfs:domain rdf:resource="http://example.org/onto/class/google_compute_image"/>
    <rdfs:range rdf:resource="http://www.w3.org/2001/XMLSchema#string"/>
  </owl:DatatypeProperty>
  <owl:DatatypeProperty rdf:about="http://example.org/onto/prop/google_compute_image_raw_key">
    <rdfs:label>raw_key</rdfs:label>
    <rdfs:comment>Specifies a 256-bit customer-supplied encryption key, encoded in
RFC 4648 base64 to either encrypt or decrypt this resource.</rdfs:comment>
    <rdfs:domain rdf:resource="http://example.org/onto/class/google_compute_image"/>
    <rdfs:range rdf:resource="http://www.w3.org/2001/XMLSchema#string"/>
  </owl:DatatypeProperty>
  <owl:DatatypeProperty rdf:about="http://example.org/onto/prop/google_compute_image_rsa_encrypted_key">
    <rdfs:label>rsa_encrypted_key</rdfs:label>
    <rdfs:comment>Specifies a 256-bit customer-supplied encryption key, encoded in
RFC 4648 base64 to either encrypt or decrypt this resource.</rdfs:comment>
    <rdfs:domain rdf:resource="http://example.org/onto/class/google_compute_image"/>
    <rdfs:range rdf:resource="http://www.w3.org/2001/XMLSchema#string"/>
  </owl:DatatypeProperty>
  <owl:DatatypeProperty rdf:about="http://example.org/onto/prop/google_compute_image_container_type">
    <rdfs:label>container_type</rdfs:label>
    <rdfs:comment>The format used to encode and transmit the block device, which
should be TAR. This is just a container and transmission format
and not a runtime format. Provided by the client when the disk
image is created. Default value: "TAR" Possible values: ["TAR"]</rdfs:comment>
    <rdfs:domain rdf:resource="http://example.org/onto/class/google_compute_image"/>
    <rdfs:range rdf:resource="http://www.w3.org/2001/XMLSchema#string"/>
  </owl:DatatypeProperty>
  <owl:DatatypeProperty rdf:about="http://example.org/onto/prop/google_compute_image_sha1">
    <rdfs:label>sha1</rdfs:label>
    <rdfs:comment>An optional SHA1 checksum of the disk image before unpackaging.
This is provided by the client when the disk image is created.</rdfs:comment>
    <rdfs:domain rdf:resource="http://example.org/onto/class/google_compute_image"/>
    <rdfs:range rdf:resource="http://www.w3.org/2001/XMLSchema#string"/>
  </owl:DatatypeProperty>
  <owl:DatatypeProperty rdf:about="http://example.org/onto/prop/google_compute_image_source">
    <rdfs:label>source</rdfs:label>
    <rdfs:comment>The full Google Cloud Storage URL where disk storage is stored
You must provide either this property or the sourceDisk property
but not both.</rdfs:comment>
    <rdfs:domain rdf:resource="http://example.org/onto/class/google_compute_image"/>
    <rdfs:range rdf:resource="http://www.w3.org/2001/XMLSchema#string"/>
  </owl:DatatypeProperty>
  <owl:DatatypeProperty rdf:about="http://example.org/onto/prop/google_compute_image_content">
    <rdfs:label>content</rdfs:label>
    <rdfs:comment>The raw content in the secure keys file.

A base64-encoded string.</rdfs:comment>
    <rdfs:domain rdf:resource="http://example.org/onto/class/google_compute_image"/>
    <rdfs:range rdf:resource="http://www.w3.org/2001/XMLSchema#string"/>
  </owl:DatatypeProperty>
  <owl:DatatypeProperty rdf:about="http://example.org/onto/prop/google_compute_image_file_type">
    <rdfs:label>file_type</rdfs:label>
    <rdfs:comment>The file type of source file.</rdfs:comment>
    <rdfs:domain rdf:resource="http://example.org/onto/class/google_compute_image"/>
    <rdfs:range rdf:resource="http://www.w3.org/2001/XMLSchema#string"/>
  </owl:DatatypeProperty>
  <owl:DatatypeProperty rdf:about="http://example.org/onto/prop/google_compute_image_content">
    <rdfs:label>content</rdfs:label>
    <rdfs:comment>The raw content in the secure keys file.

A base64-encoded string.</rdfs:comment>
    <rdfs:domain rdf:resource="http://example.org/onto/class/google_compute_image"/>
    <rdfs:range rdf:resource="http://www.w3.org/2001/XMLSchema#string"/>
  </owl:DatatypeProperty>
  <owl:DatatypeProperty rdf:about="http://example.org/onto/prop/google_compute_image_file_type">
    <rdfs:label>file_type</rdfs:label>
    <rdfs:comment>The file type of source file.</rdfs:comment>
    <rdfs:domain rdf:resource="http://example.org/onto/class/google_compute_image"/>
    <rdfs:range rdf:resource="http://www.w3.org/2001/XMLSchema#string"/>
  </owl:DatatypeProperty>
  <owl:DatatypeProperty rdf:about="http://example.org/onto/prop/google_compute_image_content">
    <rdfs:label>content</rdfs:label>
    <rdfs:comment>The raw content in the secure keys file.

A base64-encoded string.</rdfs:comment>
    <rdfs:domain rdf:resource="http://example.org/onto/class/google_compute_image"/>
    <rdfs:range rdf:resource="http://www.w3.org/2001/XMLSchema#string"/>
  </owl:DatatypeProperty>
  <owl:DatatypeProperty rdf:about="http://example.org/onto/prop/google_compute_image_file_type">
    <rdfs:label>file_type</rdfs:label>
    <rdfs:comment>The file type of source file.</rdfs:comment>
    <rdfs:domain rdf:resource="http://example.org/onto/class/google_compute_image"/>
    <rdfs:range rdf:resource="http://www.w3.org/2001/XMLSchema#string"/>
  </owl:DatatypeProperty>
  <owl:DatatypeProperty rdf:about="http://example.org/onto/prop/google_compute_image_content">
    <rdfs:label>content</rdfs:label>
    <rdfs:comment>The raw content in the secure keys file.

A base64-encoded string.</rdfs:comment>
    <rdfs:domain rdf:resource="http://example.org/onto/class/google_compute_image"/>
    <rdfs:range rdf:resource="http://www.w3.org/2001/XMLSchema#string"/>
  </owl:DatatypeProperty>
  <owl:DatatypeProperty rdf:about="http://example.org/onto/prop/google_compute_image_file_type">
    <rdfs:label>file_type</rdfs:label>
    <rdfs:comment>The file type of source file.</rdfs:comment>
    <rdfs:domain rdf:resource="http://example.org/onto/class/google_compute_image"/>
    <rdfs:range rdf:resource="http://www.w3.org/2001/XMLSchema#string"/>
  </owl:DatatypeProperty>
  <owl:DatatypeProperty rdf:about="http://example.org/onto/prop/google_compute_image_kms_key_self_link">
    <rdfs:label>kms_key_self_link</rdfs:label>
    <rdfs:comment>The self link of the encryption key used to decrypt this resource. Also called KmsKeyName
in the cloud console. Your project's Compute Engine System service account
('service-{{PROJECT_NUMBER}}@compute-system.iam.gserviceaccount.com') must have
'roles/cloudkms.cryptoKeyEncrypterDecrypter' to use this feature.
See https://cloud.google.com/compute/docs/disks/customer-managed-encryption#encrypt_a_new_persistent_disk_with_your_own_keys</rdfs:comment>
    <rdfs:domain rdf:resource="http://example.org/onto/class/google_compute_image"/>
    <rdfs:range rdf:resource="http://www.w3.org/2001/XMLSchema#string"/>
  </owl:DatatypeProperty>
  <owl:DatatypeProperty rdf:about="http://example.org/onto/prop/google_compute_image_kms_key_service_account">
    <rdfs:label>kms_key_service_account</rdfs:label>
    <rdfs:comment>The service account being used for the encryption request for the
given KMS key. If absent, the Compute Engine default service
account is used.</rdfs:comment>
    <rdfs:domain rdf:resource="http://example.org/onto/class/google_compute_image"/>
    <rdfs:range rdf:resource="http://www.w3.org/2001/XMLSchema#string"/>
  </owl:DatatypeProperty>
  <owl:DatatypeProperty rdf:about="http://example.org/onto/prop/google_compute_image_raw_key">
    <rdfs:label>raw_key</rdfs:label>
    <rdfs:comment>Specifies a 256-bit customer-supplied encryption key, encoded in
RFC 4648 base64 to either encrypt or decrypt this resource.</rdfs:comment>
    <rdfs:domain rdf:resource="http://example.org/onto/class/google_compute_image"/>
    <rdfs:range rdf:resource="http://www.w3.org/2001/XMLSchema#string"/>
  </owl:DatatypeProperty>
  <owl:DatatypeProperty rdf:about="http://example.org/onto/prop/google_compute_image_rsa_encrypted_key">
    <rdfs:label>rsa_encrypted_key</rdfs:label>
    <rdfs:comment>Specifies an RFC 4648 base64 encoded, RSA-wrapped 2048-bit
customer-supplied encryption key to either encrypt or decrypt
this resource. You can provide either the rawKey or the rsaEncryptedKey.</rdfs:comment>
    <rdfs:domain rdf:resource="http://example.org/onto/class/google_compute_image"/>
    <rdfs:range rdf:resource="http://www.w3.org/2001/XMLSchema#string"/>
  </owl:DatatypeProperty>
  <owl:DatatypeProperty rdf:about="http://example.org/onto/prop/google_compute_image_kms_key_self_link">
    <rdfs:label>kms_key_self_link</rdfs:label>
    <rdfs:comment>The self link of the encryption key used to decrypt this resource. Also called KmsKeyName
in the cloud console. Your project's Compute Engine System service account
('service-{{PROJECT_NUMBER}}@compute-system.iam.gserviceaccount.com') must have
'roles/cloudkms.cryptoKeyEncrypterDecrypter' to use this feature.
See https://cloud.google.com/compute/docs/disks/customer-managed-encryption#encrypt_a_new_persistent_disk_with_your_own_keys</rdfs:comment>
    <rdfs:domain rdf:resource="http://example.org/onto/class/google_compute_image"/>
    <rdfs:range rdf:resource="http://www.w3.org/2001/XMLSchema#string"/>
  </owl:DatatypeProperty>
  <owl:DatatypeProperty rdf:about="http://example.org/onto/prop/google_compute_image_kms_key_service_account">
    <rdfs:label>kms_key_service_account</rdfs:label>
    <rdfs:comment>The service account being used for the encryption request for the
given KMS key. If absent, the Compute Engine default service
account is used.</rdfs:comment>
    <rdfs:domain rdf:resource="http://example.org/onto/class/google_compute_image"/>
    <rdfs:range rdf:resource="http://www.w3.org/2001/XMLSchema#string"/>
  </owl:DatatypeProperty>
  <owl:DatatypeProperty rdf:about="http://example.org/onto/prop/google_compute_image_raw_key">
    <rdfs:label>raw_key</rdfs:label>
    <rdfs:comment>Specifies a 256-bit customer-supplied encryption key, encoded in
RFC 4648 base64 to either encrypt or decrypt this resource.</rdfs:comment>
    <rdfs:domain rdf:resource="http://example.org/onto/class/google_compute_image"/>
    <rdfs:range rdf:resource="http://www.w3.org/2001/XMLSchema#string"/>
  </owl:DatatypeProperty>
  <owl:DatatypeProperty rdf:about="http://example.org/onto/prop/google_compute_image_rsa_encrypted_key">
    <rdfs:label>rsa_encrypted_key</rdfs:label>
    <rdfs:comment>Specifies an RFC 4648 base64 encoded, RSA-wrapped 2048-bit
customer-supplied encryption key to either encrypt or decrypt
this resource. You can provide either the rawKey or the rsaEncryptedKey.</rdfs:comment>
    <rdfs:domain rdf:resource="http://example.org/onto/class/google_compute_image"/>
    <rdfs:range rdf:resource="http://www.w3.org/2001/XMLSchema#string"/>
  </owl:DatatypeProperty>
  <owl:DatatypeProperty rdf:about="http://example.org/onto/prop/google_compute_image_kms_key_self_link">
    <rdfs:label>kms_key_self_link</rdfs:label>
    <rdfs:comment>The self link of the encryption key used to decrypt this resource. Also called KmsKeyName
in the cloud console. Your project's Compute Engine System service account
('service-{{PROJECT_NUMBER}}@compute-system.iam.gserviceaccount.com') must have
'roles/cloudkms.cryptoKeyEncrypterDecrypter' to use this feature.
See https://cloud.google.com/compute/docs/disks/customer-managed-encryption#encrypt_a_new_persistent_disk_with_your_own_keys</rdfs:comment>
    <rdfs:domain rdf:resource="http://example.org/onto/class/google_compute_image"/>
    <rdfs:range rdf:resource="http://www.w3.org/2001/XMLSchema#string"/>
  </owl:DatatypeProperty>
  <owl:DatatypeProperty rdf:about="http://example.org/onto/prop/google_compute_image_kms_key_service_account">
    <rdfs:label>kms_key_service_account</rdfs:label>
    <rdfs:comment>The service account being used for the encryption request for the
given KMS key. If absent, the Compute Engine default service
account is used.</rdfs:comment>
    <rdfs:domain rdf:resource="http://example.org/onto/class/google_compute_image"/>
    <rdfs:range rdf:resource="http://www.w3.org/2001/XMLSchema#string"/>
  </owl:DatatypeProperty>
  <owl:DatatypeProperty rdf:about="http://example.org/onto/prop/google_compute_image_raw_key">
    <rdfs:label>raw_key</rdfs:label>
    <rdfs:comment>Specifies a 256-bit customer-supplied encryption key, encoded in
RFC 4648 base64 to either encrypt or decrypt this resource.</rdfs:comment>
    <rdfs:domain rdf:resource="http://example.org/onto/class/google_compute_image"/>
    <rdfs:range rdf:resource="http://www.w3.org/2001/XMLSchema#string"/>
  </owl:DatatypeProperty>
  <owl:DatatypeProperty rdf:about="http://example.org/onto/prop/google_compute_image_rsa_encrypted_key">
    <rdfs:label>rsa_encrypted_key</rdfs:label>
    <rdfs:comment>Specifies an RFC 4648 base64 encoded, RSA-wrapped 2048-bit
customer-supplied encryption key to either encrypt or decrypt
this resource. You can provide either the rawKey or the rsaEncryptedKey.</rdfs:comment>
    <rdfs:domain rdf:resource="http://example.org/onto/class/google_compute_image"/>
    <rdfs:range rdf:resource="http://www.w3.org/2001/XMLSchema#string"/>
  </owl:DatatypeProperty>
  <owl:DatatypeProperty rdf:about="http://example.org/onto/prop/google_compute_image_create">
    <rdfs:label>create</rdfs:label>
    <rdfs:domain rdf:resource="http://example.org/onto/class/google_compute_image"/>
    <rdfs:range rdf:resource="http://www.w3.org/2001/XMLSchema#string"/>
  </owl:DatatypeProperty>
  <owl:DatatypeProperty rdf:about="http://example.org/onto/prop/google_compute_image_delete">
    <rdfs:label>delete</rdfs:label>
    <rdfs:domain rdf:resource="http://example.org/onto/class/google_compute_image"/>
    <rdfs:range rdf:resource="http://www.w3.org/2001/XMLSchema#string"/>
  </owl:DatatypeProperty>
  <owl:DatatypeProperty rdf:about="http://example.org/onto/prop/google_compute_image_update">
    <rdfs:label>update</rdfs:label>
    <rdfs:domain rdf:resource="http://example.org/onto/class/google_compute_image"/>
    <rdfs:range rdf:resource="http://www.w3.org/2001/XMLSchema#string"/>
  </owl:DatatypeProperty>
</rdf:RDF>
