<?xml version="1.0" encoding="UTF-8"?>
<rdf:RDF
  xmlns:rdf="http://www.w3.org/1999/02/22-rdf-syntax-ns#"
  xmlns:rdfs="http://www.w3.org/2000/01/rdf-schema#"
  xmlns:owl="http://www.w3.org/2002/07/owl#"
  xmlns:xsd="http://www.w3.org/2001/XMLSchema#"
  xml:base="http://example.org/onto/">
  <owl:Class rdf:about="http://example.org/onto/class/google_discovery_engine_recommendation_engine">
    <rdfs:label>google_discovery_engine_recommendation_engine</rdfs:label>
    <rdfs:comment>#
#     ***     AUTO GENERATED CODE    ***    Type: MMv1     ***
#
# ----------------------------------------------------------------------------
#
#     This code is generated by Magic Modules using the following:
#
#     Configuration: https:#github.com/GoogleCloudPlatform/magic-modules/tree/main/mmv1/products/discoveryengine/RecommendationEngine.yaml
#     Template:      https:#github.com/GoogleCloudPlatform/magic-modules/tree/main/mmv1/templates/terraform/resource.html.markdown.tmpl
#
#     DO NOT EDIT this file directly. Any changes made to this file will be
#     overwritten during the next generation cycle.
#
# ----------------------------------------------------------------------------
subcategory: "Discovery Engine"
description: |-
  Vertex AI Search recommendation apps.
---</rdfs:comment>
  </owl:Class>
  <owl:DatatypeProperty rdf:about="http://example.org/onto/prop/google_discovery_engine_recommendation_engine_create_time">
    <rdfs:label>create_time</rdfs:label>
    <rdfs:comment>Timestamp the Engine was created at.</rdfs:comment>
    <rdfs:domain rdf:resource="http://example.org/onto/class/google_discovery_engine_recommendation_engine"/>
    <rdfs:range rdf:resource="http://www.w3.org/2001/XMLSchema#string"/>
  </owl:DatatypeProperty>
  <owl:DatatypeProperty rdf:about="http://example.org/onto/prop/google_discovery_engine_recommendation_engine_data_store_ids">
    <rdfs:label>data_store_ids</rdfs:label>
    <rdfs:comment>The data stores associated with this engine. For SOLUTION_TYPE_RECOMMENDATION type of engines, they can only associate with at most one data store.</rdfs:comment>
    <rdfs:domain rdf:resource="http://example.org/onto/class/google_discovery_engine_recommendation_engine"/>
    <rdfs:range rdf:resource="http://www.w3.org/2001/XMLSchema#string"/>
  </owl:DatatypeProperty>
  <owl:DatatypeProperty rdf:about="http://example.org/onto/prop/google_discovery_engine_recommendation_engine_display_name">
    <rdfs:label>display_name</rdfs:label>
    <rdfs:comment>Required. The display name of the engine. Should be human readable. UTF-8 encoded string with limit of 1024 characters.</rdfs:comment>
    <rdfs:domain rdf:resource="http://example.org/onto/class/google_discovery_engine_recommendation_engine"/>
    <rdfs:range rdf:resource="http://www.w3.org/2001/XMLSchema#string"/>
  </owl:DatatypeProperty>
  <owl:DatatypeProperty rdf:about="http://example.org/onto/prop/google_discovery_engine_recommendation_engine_engine_id">
    <rdfs:label>engine_id</rdfs:label>
    <rdfs:comment>Unique ID to use for Recommendation Engine.</rdfs:comment>
    <rdfs:domain rdf:resource="http://example.org/onto/class/google_discovery_engine_recommendation_engine"/>
    <rdfs:range rdf:resource="http://www.w3.org/2001/XMLSchema#string"/>
  </owl:DatatypeProperty>
  <owl:DatatypeProperty rdf:about="http://example.org/onto/prop/google_discovery_engine_recommendation_engine_id">
    <rdfs:label>id</rdfs:label>
    <rdfs:domain rdf:resource="http://example.org/onto/class/google_discovery_engine_recommendation_engine"/>
    <rdfs:range rdf:resource="http://www.w3.org/2001/XMLSchema#string"/>
  </owl:DatatypeProperty>
  <owl:DatatypeProperty rdf:about="http://example.org/onto/prop/google_discovery_engine_recommendation_engine_industry_vertical">
    <rdfs:label>industry_vertical</rdfs:label>
    <rdfs:comment>The industry vertical that the engine registers. The restriction of the Engine industry vertical is based on DataStore: If unspecified, default to GENERIC. Vertical on Engine has to match vertical of the DataStore liniked to the engine. Default value: "GENERIC" Possible values: ["GENERIC", "MEDIA"]</rdfs:comment>
    <rdfs:domain rdf:resource="http://example.org/onto/class/google_discovery_engine_recommendation_engine"/>
    <rdfs:range rdf:resource="http://www.w3.org/2001/XMLSchema#string"/>
  </owl:DatatypeProperty>
  <owl:DatatypeProperty rdf:about="http://example.org/onto/prop/google_discovery_engine_recommendation_engine_location">
    <rdfs:label>location</rdfs:label>
    <rdfs:comment>The geographic location where the data store should reside. The value can
only be one of "global", "us" and "eu".</rdfs:comment>
    <rdfs:domain rdf:resource="http://example.org/onto/class/google_discovery_engine_recommendation_engine"/>
    <rdfs:range rdf:resource="http://www.w3.org/2001/XMLSchema#string"/>
  </owl:DatatypeProperty>
  <owl:DatatypeProperty rdf:about="http://example.org/onto/prop/google_discovery_engine_recommendation_engine_name">
    <rdfs:label>name</rdfs:label>
    <rdfs:comment>The unique full resource name of the recommendation engine. Values are of the format
'projects/{project}/locations/{location}/collections/{collection}/engines/{engine_id}'.
This field must be a UTF-8 encoded string with a length limit of 1024 characters.</rdfs:comment>
    <rdfs:domain rdf:resource="http://example.org/onto/class/google_discovery_engine_recommendation_engine"/>
    <rdfs:range rdf:resource="http://www.w3.org/2001/XMLSchema#string"/>
  </owl:DatatypeProperty>
  <owl:DatatypeProperty rdf:about="http://example.org/onto/prop/google_discovery_engine_recommendation_engine_project">
    <rdfs:label>project</rdfs:label>
    <rdfs:domain rdf:resource="http://example.org/onto/class/google_discovery_engine_recommendation_engine"/>
    <rdfs:range rdf:resource="http://www.w3.org/2001/XMLSchema#string"/>
  </owl:DatatypeProperty>
  <owl:DatatypeProperty rdf:about="http://example.org/onto/prop/google_discovery_engine_recommendation_engine_update_time">
    <rdfs:label>update_time</rdfs:label>
    <rdfs:comment>Timestamp the Engine was last updated.</rdfs:comment>
    <rdfs:domain rdf:resource="http://example.org/onto/class/google_discovery_engine_recommendation_engine"/>
    <rdfs:range rdf:resource="http://www.w3.org/2001/XMLSchema#string"/>
  </owl:DatatypeProperty>
  <owl:DatatypeProperty rdf:about="http://example.org/onto/prop/google_discovery_engine_recommendation_engine_company_name">
    <rdfs:label>company_name</rdfs:label>
    <rdfs:comment>The name of the company, business or entity that is associated with the engine. Setting this may help improve LLM related features.cd</rdfs:comment>
    <rdfs:domain rdf:resource="http://example.org/onto/class/google_discovery_engine_recommendation_engine"/>
    <rdfs:range rdf:resource="http://www.w3.org/2001/XMLSchema#string"/>
  </owl:DatatypeProperty>
  <owl:DatatypeProperty rdf:about="http://example.org/onto/prop/google_discovery_engine_recommendation_engine_optimization_objective">
    <rdfs:label>optimization_objective</rdfs:label>
    <rdfs:comment>The optimization objective. e.g., 'cvr'.
This field together with MediaRecommendationEngineConfig.type describes
engine metadata to use to control engine training and serving.
Currently supported values: 'ctr', 'cvr'.
If not specified, we choose default based on engine type. Default depends on type of recommendation:
'recommended-for-you' => 'ctr'
'others-you-may-like' => 'ctr'</rdfs:comment>
    <rdfs:domain rdf:resource="http://example.org/onto/class/google_discovery_engine_recommendation_engine"/>
    <rdfs:range rdf:resource="http://www.w3.org/2001/XMLSchema#string"/>
  </owl:DatatypeProperty>
  <owl:DatatypeProperty rdf:about="http://example.org/onto/prop/google_discovery_engine_recommendation_engine_training_state">
    <rdfs:label>training_state</rdfs:label>
    <rdfs:comment>The training state that the engine is in (e.g. 'TRAINING' or 'PAUSED').
Since part of the cost of running the service
is frequency of training - this can be used to determine when to train
engine in order to control cost. If not specified: the default value for
'CreateEngine' method is 'TRAINING'. The default value for
'UpdateEngine' method is to keep the state the same as before. Possible values: ["PAUSED", "TRAINING"]</rdfs:comment>
    <rdfs:domain rdf:resource="http://example.org/onto/class/google_discovery_engine_recommendation_engine"/>
    <rdfs:range rdf:resource="http://www.w3.org/2001/XMLSchema#string"/>
  </owl:DatatypeProperty>
  <owl:DatatypeProperty rdf:about="http://example.org/onto/prop/google_discovery_engine_recommendation_engine_type">
    <rdfs:label>type</rdfs:label>
    <rdfs:comment>The type of engine. e.g., 'recommended-for-you'.
This field together with MediaRecommendationEngineConfig.optimizationObjective describes
engine metadata to use to control engine training and serving.
Currently supported values: 'recommended-for-you', 'others-you-may-like',
'more-like-this', 'most-popular-items'.</rdfs:comment>
    <rdfs:domain rdf:resource="http://example.org/onto/class/google_discovery_engine_recommendation_engine"/>
    <rdfs:range rdf:resource="http://www.w3.org/2001/XMLSchema#string"/>
  </owl:DatatypeProperty>
  <owl:DatatypeProperty rdf:about="http://example.org/onto/prop/google_discovery_engine_recommendation_engine_time_window_days">
    <rdfs:label>time_window_days</rdfs:label>
    <rdfs:comment>The time window of which the engine is queried at training and
prediction time. Positive integers only. The value translates to the
last X days of events. Currently required for the 'most-popular-items'
engine.</rdfs:comment>
    <rdfs:domain rdf:resource="http://example.org/onto/class/google_discovery_engine_recommendation_engine"/>
    <rdfs:range rdf:resource="http://www.w3.org/2001/XMLSchema#string"/>
  </owl:DatatypeProperty>
  <owl:DatatypeProperty rdf:about="http://example.org/onto/prop/google_discovery_engine_recommendation_engine_context_event_type">
    <rdfs:label>context_event_type</rdfs:label>
    <rdfs:comment>The type of event with which the engine is queried at prediction time.
If set to 'generic', only 'view-item', 'media-play',and
'media-complete' will be used as 'context-event' in engine training. If
set to 'view-home-page', 'view-home-page' will also be used as
'context-events' in addition to 'view-item', 'media-play', and
'media-complete'. Currently supported for the 'recommended-for-you'
engine. Currently supported values: 'view-home-page', 'generic'.</rdfs:comment>
    <rdfs:domain rdf:resource="http://example.org/onto/class/google_discovery_engine_recommendation_engine"/>
    <rdfs:range rdf:resource="http://www.w3.org/2001/XMLSchema#string"/>
  </owl:DatatypeProperty>
  <owl:DatatypeProperty rdf:about="http://example.org/onto/prop/google_discovery_engine_recommendation_engine_target_field">
    <rdfs:label>target_field</rdfs:label>
    <rdfs:comment>The name of the field to target. Currently supported values: 'watch-percentage', 'watch-time'.</rdfs:comment>
    <rdfs:domain rdf:resource="http://example.org/onto/class/google_discovery_engine_recommendation_engine"/>
    <rdfs:range rdf:resource="http://www.w3.org/2001/XMLSchema#string"/>
  </owl:DatatypeProperty>
  <owl:DatatypeProperty rdf:about="http://example.org/onto/prop/google_discovery_engine_recommendation_engine_target_field_value_float">
    <rdfs:label>target_field_value_float</rdfs:label>
    <rdfs:comment>The threshold to be applied to the target (e.g., 0.5).</rdfs:comment>
    <rdfs:domain rdf:resource="http://example.org/onto/class/google_discovery_engine_recommendation_engine"/>
    <rdfs:range rdf:resource="http://www.w3.org/2001/XMLSchema#string"/>
  </owl:DatatypeProperty>
  <owl:DatatypeProperty rdf:about="http://example.org/onto/prop/google_discovery_engine_recommendation_engine_create">
    <rdfs:label>create</rdfs:label>
    <rdfs:domain rdf:resource="http://example.org/onto/class/google_discovery_engine_recommendation_engine"/>
    <rdfs:range rdf:resource="http://www.w3.org/2001/XMLSchema#string"/>
  </owl:DatatypeProperty>
  <owl:DatatypeProperty rdf:about="http://example.org/onto/prop/google_discovery_engine_recommendation_engine_delete">
    <rdfs:label>delete</rdfs:label>
    <rdfs:domain rdf:resource="http://example.org/onto/class/google_discovery_engine_recommendation_engine"/>
    <rdfs:range rdf:resource="http://www.w3.org/2001/XMLSchema#string"/>
  </owl:DatatypeProperty>
  <owl:DatatypeProperty rdf:about="http://example.org/onto/prop/google_discovery_engine_recommendation_engine_update">
    <rdfs:label>update</rdfs:label>
    <rdfs:domain rdf:resource="http://example.org/onto/class/google_discovery_engine_recommendation_engine"/>
    <rdfs:range rdf:resource="http://www.w3.org/2001/XMLSchema#string"/>
  </owl:DatatypeProperty>
</rdf:RDF>
