<?xml version="1.0" encoding="UTF-8"?>
<rdf:RDF
  xmlns:rdf="http://www.w3.org/1999/02/22-rdf-syntax-ns#"
  xmlns:rdfs="http://www.w3.org/2000/01/rdf-schema#"
  xmlns:owl="http://www.w3.org/2002/07/owl#"
  xmlns:xsd="http://www.w3.org/2001/XMLSchema#"
  xml:base="http://example.org/onto/">
  <owl:Class rdf:about="http://example.org/onto/class/google_dataflow_job">
    <rdfs:label>google_dataflow_job</rdfs:label>
    <rdfs:comment>#
#     ***     AUTO GENERATED CODE    ***    Type: Handwritten     ***
#
# ----------------------------------------------------------------------------
#
#     This code is generated by Magic Modules using the following:
#
#     Source file: https://github.com/GoogleCloudPlatform/magic-modules/tree/main/mmv1/third_party/terraform/website/docs/r/dataflow_job.html.markdown
#
#     DO NOT EDIT this file directly. Any changes made to this file will be
#     overwritten during the next generation cycle.
#
# ----------------------------------------------------------------------------
subcategory: "Dataflow"
description: |-
  Creates a job in Dataflow according to a provided config file.
---</rdfs:comment>
  </owl:Class>
  <owl:DatatypeProperty rdf:about="http://example.org/onto/prop/google_dataflow_job_additional_experiments">
    <rdfs:label>additional_experiments</rdfs:label>
    <rdfs:comment>List of experiments that should be used by the job. An example value is ["enable_stackdriver_agent_metrics"].</rdfs:comment>
    <rdfs:domain rdf:resource="http://example.org/onto/class/google_dataflow_job"/>
    <rdfs:range rdf:resource="http://www.w3.org/2001/XMLSchema#string"/>
  </owl:DatatypeProperty>
  <owl:DatatypeProperty rdf:about="http://example.org/onto/prop/google_dataflow_job_effective_labels">
    <rdfs:label>effective_labels</rdfs:label>
    <rdfs:comment>All of labels (key/value pairs) present on the resource in GCP, including the labels configured through Terraform, other clients and services.</rdfs:comment>
    <rdfs:domain rdf:resource="http://example.org/onto/class/google_dataflow_job"/>
    <rdfs:range rdf:resource="http://www.w3.org/2001/XMLSchema#string"/>
  </owl:DatatypeProperty>
  <owl:DatatypeProperty rdf:about="http://example.org/onto/prop/google_dataflow_job_enable_streaming_engine">
    <rdfs:label>enable_streaming_engine</rdfs:label>
    <rdfs:comment>Indicates if the job should use the streaming engine feature.</rdfs:comment>
    <rdfs:domain rdf:resource="http://example.org/onto/class/google_dataflow_job"/>
    <rdfs:range rdf:resource="http://www.w3.org/2001/XMLSchema#string"/>
  </owl:DatatypeProperty>
  <owl:DatatypeProperty rdf:about="http://example.org/onto/prop/google_dataflow_job_id">
    <rdfs:label>id</rdfs:label>
    <rdfs:domain rdf:resource="http://example.org/onto/class/google_dataflow_job"/>
    <rdfs:range rdf:resource="http://www.w3.org/2001/XMLSchema#string"/>
  </owl:DatatypeProperty>
  <owl:DatatypeProperty rdf:about="http://example.org/onto/prop/google_dataflow_job_ip_configuration">
    <rdfs:label>ip_configuration</rdfs:label>
    <rdfs:comment>The configuration for VM IPs. Options are "WORKER_IP_PUBLIC" or "WORKER_IP_PRIVATE".</rdfs:comment>
    <rdfs:domain rdf:resource="http://example.org/onto/class/google_dataflow_job"/>
    <rdfs:range rdf:resource="http://www.w3.org/2001/XMLSchema#string"/>
  </owl:DatatypeProperty>
  <owl:DatatypeProperty rdf:about="http://example.org/onto/prop/google_dataflow_job_job_id">
    <rdfs:label>job_id</rdfs:label>
    <rdfs:comment>The unique ID of this job.</rdfs:comment>
    <rdfs:domain rdf:resource="http://example.org/onto/class/google_dataflow_job"/>
    <rdfs:range rdf:resource="http://www.w3.org/2001/XMLSchema#string"/>
  </owl:DatatypeProperty>
  <owl:DatatypeProperty rdf:about="http://example.org/onto/prop/google_dataflow_job_kms_key_name">
    <rdfs:label>kms_key_name</rdfs:label>
    <rdfs:comment>The name for the Cloud KMS key for the job. Key format is: projects/PROJECT_ID/locations/LOCATION/keyRings/KEY_RING/cryptoKeys/KEY</rdfs:comment>
    <rdfs:domain rdf:resource="http://example.org/onto/class/google_dataflow_job"/>
    <rdfs:range rdf:resource="http://www.w3.org/2001/XMLSchema#string"/>
  </owl:DatatypeProperty>
  <owl:DatatypeProperty rdf:about="http://example.org/onto/prop/google_dataflow_job_labels">
    <rdfs:label>labels</rdfs:label>
    <rdfs:comment>User labels to be specified for the job. Keys and values should follow the restrictions specified in the labeling restrictions page. NOTE: This field is non-authoritative, and will only manage the labels present in your configuration.
				Please refer to the field 'effective_labels' for all of the labels present on the resource.</rdfs:comment>
    <rdfs:domain rdf:resource="http://example.org/onto/class/google_dataflow_job"/>
    <rdfs:range rdf:resource="http://www.w3.org/2001/XMLSchema#string"/>
  </owl:DatatypeProperty>
  <owl:DatatypeProperty rdf:about="http://example.org/onto/prop/google_dataflow_job_machine_type">
    <rdfs:label>machine_type</rdfs:label>
    <rdfs:comment>The machine type to use for the job.</rdfs:comment>
    <rdfs:domain rdf:resource="http://example.org/onto/class/google_dataflow_job"/>
    <rdfs:range rdf:resource="http://www.w3.org/2001/XMLSchema#string"/>
  </owl:DatatypeProperty>
  <owl:DatatypeProperty rdf:about="http://example.org/onto/prop/google_dataflow_job_max_workers">
    <rdfs:label>max_workers</rdfs:label>
    <rdfs:comment>The number of workers permitted to work on the job. More workers may improve processing speed at additional cost.</rdfs:comment>
    <rdfs:domain rdf:resource="http://example.org/onto/class/google_dataflow_job"/>
    <rdfs:range rdf:resource="http://www.w3.org/2001/XMLSchema#string"/>
  </owl:DatatypeProperty>
  <owl:DatatypeProperty rdf:about="http://example.org/onto/prop/google_dataflow_job_name">
    <rdfs:label>name</rdfs:label>
    <rdfs:comment>A unique name for the resource, required by Dataflow.</rdfs:comment>
    <rdfs:domain rdf:resource="http://example.org/onto/class/google_dataflow_job"/>
    <rdfs:range rdf:resource="http://www.w3.org/2001/XMLSchema#string"/>
  </owl:DatatypeProperty>
  <owl:DatatypeProperty rdf:about="http://example.org/onto/prop/google_dataflow_job_network">
    <rdfs:label>network</rdfs:label>
    <rdfs:comment>The network to which VMs will be assigned. If it is not provided, "default" will be used.</rdfs:comment>
    <rdfs:domain rdf:resource="http://example.org/onto/class/google_dataflow_job"/>
    <rdfs:range rdf:resource="http://www.w3.org/2001/XMLSchema#string"/>
  </owl:DatatypeProperty>
  <owl:DatatypeProperty rdf:about="http://example.org/onto/prop/google_dataflow_job_on_delete">
    <rdfs:label>on_delete</rdfs:label>
    <rdfs:comment>One of "drain" or "cancel". Specifies behavior of deletion during terraform destroy.</rdfs:comment>
    <rdfs:domain rdf:resource="http://example.org/onto/class/google_dataflow_job"/>
    <rdfs:range rdf:resource="http://www.w3.org/2001/XMLSchema#string"/>
  </owl:DatatypeProperty>
  <owl:DatatypeProperty rdf:about="http://example.org/onto/prop/google_dataflow_job_parameters">
    <rdfs:label>parameters</rdfs:label>
    <rdfs:comment>Key/Value pairs to be passed to the Dataflow job (as used in the template).</rdfs:comment>
    <rdfs:domain rdf:resource="http://example.org/onto/class/google_dataflow_job"/>
    <rdfs:range rdf:resource="http://www.w3.org/2001/XMLSchema#string"/>
  </owl:DatatypeProperty>
  <owl:DatatypeProperty rdf:about="http://example.org/onto/prop/google_dataflow_job_project">
    <rdfs:label>project</rdfs:label>
    <rdfs:comment>The project in which the resource belongs.</rdfs:comment>
    <rdfs:domain rdf:resource="http://example.org/onto/class/google_dataflow_job"/>
    <rdfs:range rdf:resource="http://www.w3.org/2001/XMLSchema#string"/>
  </owl:DatatypeProperty>
  <owl:DatatypeProperty rdf:about="http://example.org/onto/prop/google_dataflow_job_region">
    <rdfs:label>region</rdfs:label>
    <rdfs:comment>The region in which the created job should run.</rdfs:comment>
    <rdfs:domain rdf:resource="http://example.org/onto/class/google_dataflow_job"/>
    <rdfs:range rdf:resource="http://www.w3.org/2001/XMLSchema#string"/>
  </owl:DatatypeProperty>
  <owl:DatatypeProperty rdf:about="http://example.org/onto/prop/google_dataflow_job_service_account_email">
    <rdfs:label>service_account_email</rdfs:label>
    <rdfs:comment>The Service Account email used to create the job.</rdfs:comment>
    <rdfs:domain rdf:resource="http://example.org/onto/class/google_dataflow_job"/>
    <rdfs:range rdf:resource="http://www.w3.org/2001/XMLSchema#string"/>
  </owl:DatatypeProperty>
  <owl:DatatypeProperty rdf:about="http://example.org/onto/prop/google_dataflow_job_skip_wait_on_job_termination">
    <rdfs:label>skip_wait_on_job_termination</rdfs:label>
    <rdfs:comment>If true, treat DRAINING and CANCELLING as terminal job states and do not wait for further changes before removing from terraform state and moving on. WARNING: this will lead to job name conflicts if you do not ensure that the job names are different, e.g. by embedding a release ID or by using a random_id.</rdfs:comment>
    <rdfs:domain rdf:resource="http://example.org/onto/class/google_dataflow_job"/>
    <rdfs:range rdf:resource="http://www.w3.org/2001/XMLSchema#string"/>
  </owl:DatatypeProperty>
  <owl:DatatypeProperty rdf:about="http://example.org/onto/prop/google_dataflow_job_state">
    <rdfs:label>state</rdfs:label>
    <rdfs:comment>The current state of the resource, selected from the JobState enum.</rdfs:comment>
    <rdfs:domain rdf:resource="http://example.org/onto/class/google_dataflow_job"/>
    <rdfs:range rdf:resource="http://www.w3.org/2001/XMLSchema#string"/>
  </owl:DatatypeProperty>
  <owl:DatatypeProperty rdf:about="http://example.org/onto/prop/google_dataflow_job_subnetwork">
    <rdfs:label>subnetwork</rdfs:label>
    <rdfs:comment>The subnetwork to which VMs will be assigned. Should be of the form "regions/REGION/subnetworks/SUBNETWORK".</rdfs:comment>
    <rdfs:domain rdf:resource="http://example.org/onto/class/google_dataflow_job"/>
    <rdfs:range rdf:resource="http://www.w3.org/2001/XMLSchema#string"/>
  </owl:DatatypeProperty>
  <owl:DatatypeProperty rdf:about="http://example.org/onto/prop/google_dataflow_job_temp_gcs_location">
    <rdfs:label>temp_gcs_location</rdfs:label>
    <rdfs:comment>A writeable location on Google Cloud Storage for the Dataflow job to dump its temporary data.</rdfs:comment>
    <rdfs:domain rdf:resource="http://example.org/onto/class/google_dataflow_job"/>
    <rdfs:range rdf:resource="http://www.w3.org/2001/XMLSchema#string"/>
  </owl:DatatypeProperty>
  <owl:DatatypeProperty rdf:about="http://example.org/onto/prop/google_dataflow_job_template_gcs_path">
    <rdfs:label>template_gcs_path</rdfs:label>
    <rdfs:comment>The Google Cloud Storage path to the Dataflow job template.</rdfs:comment>
    <rdfs:domain rdf:resource="http://example.org/onto/class/google_dataflow_job"/>
    <rdfs:range rdf:resource="http://www.w3.org/2001/XMLSchema#string"/>
  </owl:DatatypeProperty>
  <owl:DatatypeProperty rdf:about="http://example.org/onto/prop/google_dataflow_job_terraform_labels">
    <rdfs:label>terraform_labels</rdfs:label>
    <rdfs:comment>The combination of labels configured directly on the resource and default labels configured on the provider.</rdfs:comment>
    <rdfs:domain rdf:resource="http://example.org/onto/class/google_dataflow_job"/>
    <rdfs:range rdf:resource="http://www.w3.org/2001/XMLSchema#string"/>
  </owl:DatatypeProperty>
  <owl:DatatypeProperty rdf:about="http://example.org/onto/prop/google_dataflow_job_transform_name_mapping">
    <rdfs:label>transform_name_mapping</rdfs:label>
    <rdfs:comment>Only applicable when updating a pipeline. Map of transform name prefixes of the job to be replaced with the corresponding name prefixes of the new job.</rdfs:comment>
    <rdfs:domain rdf:resource="http://example.org/onto/class/google_dataflow_job"/>
    <rdfs:range rdf:resource="http://www.w3.org/2001/XMLSchema#string"/>
  </owl:DatatypeProperty>
  <owl:DatatypeProperty rdf:about="http://example.org/onto/prop/google_dataflow_job_type">
    <rdfs:label>type</rdfs:label>
    <rdfs:comment>The type of this job, selected from the JobType enum.</rdfs:comment>
    <rdfs:domain rdf:resource="http://example.org/onto/class/google_dataflow_job"/>
    <rdfs:range rdf:resource="http://www.w3.org/2001/XMLSchema#string"/>
  </owl:DatatypeProperty>
  <owl:DatatypeProperty rdf:about="http://example.org/onto/prop/google_dataflow_job_zone">
    <rdfs:label>zone</rdfs:label>
    <rdfs:comment>The zone in which the created job should run. If it is not provided, the provider zone is used.</rdfs:comment>
    <rdfs:domain rdf:resource="http://example.org/onto/class/google_dataflow_job"/>
    <rdfs:range rdf:resource="http://www.w3.org/2001/XMLSchema#string"/>
  </owl:DatatypeProperty>
  <owl:DatatypeProperty rdf:about="http://example.org/onto/prop/google_dataflow_job_update">
    <rdfs:label>update</rdfs:label>
    <rdfs:domain rdf:resource="http://example.org/onto/class/google_dataflow_job"/>
    <rdfs:range rdf:resource="http://www.w3.org/2001/XMLSchema#string"/>
  </owl:DatatypeProperty>
</rdf:RDF>
