<?xml version="1.0" encoding="UTF-8"?>
<rdf:RDF
  xmlns:rdf="http://www.w3.org/1999/02/22-rdf-syntax-ns#"
  xmlns:rdfs="http://www.w3.org/2000/01/rdf-schema#"
  xmlns:owl="http://www.w3.org/2002/07/owl#"
  xmlns:xsd="http://www.w3.org/2001/XMLSchema#"
  xml:base="http://example.org/onto/">
  <owl:Class rdf:about="http://example.org/onto/class/google_network_services_edge_cache_keyset">
    <rdfs:label>google_network_services_edge_cache_keyset</rdfs:label>
    <rdfs:comment>#
#     ***     AUTO GENERATED CODE    ***    Type: MMv1     ***
#
# ----------------------------------------------------------------------------
#
#     This code is generated by Magic Modules using the following:
#
#     Configuration: https:#github.com/GoogleCloudPlatform/magic-modules/tree/main/mmv1/products/networkservices/EdgeCacheKeyset.yaml
#     Template:      https:#github.com/GoogleCloudPlatform/magic-modules/tree/main/mmv1/templates/terraform/resource.html.markdown.tmpl
#
#     DO NOT EDIT this file directly. Any changes made to this file will be
#     overwritten during the next generation cycle.
#
# ----------------------------------------------------------------------------
subcategory: "Network Services"
description: |-
  EdgeCacheKeyset represents a collection of public keys used for validating signed requests.
---</rdfs:comment>
  </owl:Class>
  <owl:DatatypeProperty rdf:about="http://example.org/onto/prop/google_network_services_edge_cache_keyset_description">
    <rdfs:label>description</rdfs:label>
    <rdfs:comment>A human-readable description of the resource.</rdfs:comment>
    <rdfs:domain rdf:resource="http://example.org/onto/class/google_network_services_edge_cache_keyset"/>
    <rdfs:range rdf:resource="http://www.w3.org/2001/XMLSchema#string"/>
  </owl:DatatypeProperty>
  <owl:DatatypeProperty rdf:about="http://example.org/onto/prop/google_network_services_edge_cache_keyset_effective_labels">
    <rdfs:label>effective_labels</rdfs:label>
    <rdfs:comment>All of labels (key/value pairs) present on the resource in GCP, including the labels configured through Terraform, other clients and services.</rdfs:comment>
    <rdfs:domain rdf:resource="http://example.org/onto/class/google_network_services_edge_cache_keyset"/>
    <rdfs:range rdf:resource="http://www.w3.org/2001/XMLSchema#string"/>
  </owl:DatatypeProperty>
  <owl:DatatypeProperty rdf:about="http://example.org/onto/prop/google_network_services_edge_cache_keyset_id">
    <rdfs:label>id</rdfs:label>
    <rdfs:domain rdf:resource="http://example.org/onto/class/google_network_services_edge_cache_keyset"/>
    <rdfs:range rdf:resource="http://www.w3.org/2001/XMLSchema#string"/>
  </owl:DatatypeProperty>
  <owl:DatatypeProperty rdf:about="http://example.org/onto/prop/google_network_services_edge_cache_keyset_labels">
    <rdfs:label>labels</rdfs:label>
    <rdfs:comment>Set of label tags associated with the EdgeCache resource.

**Note**: This field is non-authoritative, and will only manage the labels present in your configuration.
Please refer to the field 'effective_labels' for all of the labels present on the resource.</rdfs:comment>
    <rdfs:domain rdf:resource="http://example.org/onto/class/google_network_services_edge_cache_keyset"/>
    <rdfs:range rdf:resource="http://www.w3.org/2001/XMLSchema#string"/>
  </owl:DatatypeProperty>
  <owl:DatatypeProperty rdf:about="http://example.org/onto/prop/google_network_services_edge_cache_keyset_name">
    <rdfs:label>name</rdfs:label>
    <rdfs:comment>Name of the resource; provided by the client when the resource is created.
The name must be 1-64 characters long, and match the regular expression [a-zA-Z][a-zA-Z0-9_-]* which means the first character must be a letter,
and all following characters must be a dash, underscore, letter or digit.</rdfs:comment>
    <rdfs:domain rdf:resource="http://example.org/onto/class/google_network_services_edge_cache_keyset"/>
    <rdfs:range rdf:resource="http://www.w3.org/2001/XMLSchema#string"/>
  </owl:DatatypeProperty>
  <owl:DatatypeProperty rdf:about="http://example.org/onto/prop/google_network_services_edge_cache_keyset_project">
    <rdfs:label>project</rdfs:label>
    <rdfs:domain rdf:resource="http://example.org/onto/class/google_network_services_edge_cache_keyset"/>
    <rdfs:range rdf:resource="http://www.w3.org/2001/XMLSchema#string"/>
  </owl:DatatypeProperty>
  <owl:DatatypeProperty rdf:about="http://example.org/onto/prop/google_network_services_edge_cache_keyset_terraform_labels">
    <rdfs:label>terraform_labels</rdfs:label>
    <rdfs:comment>The combination of labels configured directly on the resource
 and default labels configured on the provider.</rdfs:comment>
    <rdfs:domain rdf:resource="http://example.org/onto/class/google_network_services_edge_cache_keyset"/>
    <rdfs:range rdf:resource="http://www.w3.org/2001/XMLSchema#string"/>
  </owl:DatatypeProperty>
  <owl:DatatypeProperty rdf:about="http://example.org/onto/prop/google_network_services_edge_cache_keyset_id">
    <rdfs:label>id</rdfs:label>
    <rdfs:comment>The ID of the public key. The ID must be 1-63 characters long, and comply with RFC1035.
The name must be 1-64 characters long, and match the regular expression [a-zA-Z][a-zA-Z0-9_-]*
which means the first character must be a letter, and all following characters must be a dash, underscore, letter or digit.</rdfs:comment>
    <rdfs:domain rdf:resource="http://example.org/onto/class/google_network_services_edge_cache_keyset"/>
    <rdfs:range rdf:resource="http://www.w3.org/2001/XMLSchema#string"/>
  </owl:DatatypeProperty>
  <owl:DatatypeProperty rdf:about="http://example.org/onto/prop/google_network_services_edge_cache_keyset_managed">
    <rdfs:label>managed</rdfs:label>
    <rdfs:comment>Set to true to have the CDN automatically manage this public key value.</rdfs:comment>
    <rdfs:domain rdf:resource="http://example.org/onto/class/google_network_services_edge_cache_keyset"/>
    <rdfs:range rdf:resource="http://www.w3.org/2001/XMLSchema#string"/>
  </owl:DatatypeProperty>
  <owl:DatatypeProperty rdf:about="http://example.org/onto/prop/google_network_services_edge_cache_keyset_value">
    <rdfs:label>value</rdfs:label>
    <rdfs:comment>The base64-encoded value of the Ed25519 public key. The base64 encoding can be padded (44 bytes) or unpadded (43 bytes).
Representations or encodings of the public key other than this will be rejected with an error.</rdfs:comment>
    <rdfs:domain rdf:resource="http://example.org/onto/class/google_network_services_edge_cache_keyset"/>
    <rdfs:range rdf:resource="http://www.w3.org/2001/XMLSchema#string"/>
  </owl:DatatypeProperty>
  <owl:DatatypeProperty rdf:about="http://example.org/onto/prop/google_network_services_edge_cache_keyset_create">
    <rdfs:label>create</rdfs:label>
    <rdfs:domain rdf:resource="http://example.org/onto/class/google_network_services_edge_cache_keyset"/>
    <rdfs:range rdf:resource="http://www.w3.org/2001/XMLSchema#string"/>
  </owl:DatatypeProperty>
  <owl:DatatypeProperty rdf:about="http://example.org/onto/prop/google_network_services_edge_cache_keyset_delete">
    <rdfs:label>delete</rdfs:label>
    <rdfs:domain rdf:resource="http://example.org/onto/class/google_network_services_edge_cache_keyset"/>
    <rdfs:range rdf:resource="http://www.w3.org/2001/XMLSchema#string"/>
  </owl:DatatypeProperty>
  <owl:DatatypeProperty rdf:about="http://example.org/onto/prop/google_network_services_edge_cache_keyset_update">
    <rdfs:label>update</rdfs:label>
    <rdfs:domain rdf:resource="http://example.org/onto/class/google_network_services_edge_cache_keyset"/>
    <rdfs:range rdf:resource="http://www.w3.org/2001/XMLSchema#string"/>
  </owl:DatatypeProperty>
  <owl:DatatypeProperty rdf:about="http://example.org/onto/prop/google_network_services_edge_cache_keyset_secret_version">
    <rdfs:label>secret_version</rdfs:label>
    <rdfs:comment>The name of the secret version in Secret Manager.

The resource name of the secret version must be in the format 'projects/*/secrets/*/versions/*' where the '*' values are replaced by the secrets themselves.
The secrets must be at least 16 bytes large.  The recommended secret size depends on the signature algorithm you are using.
* If you are using HMAC-SHA1, we suggest 20-byte secrets.
* If you are using HMAC-SHA256, we suggest 32-byte secrets.
See RFC 2104, Section 3 for more details on these recommendations.</rdfs:comment>
    <rdfs:domain rdf:resource="http://example.org/onto/class/google_network_services_edge_cache_keyset"/>
    <rdfs:range rdf:resource="http://www.w3.org/2001/XMLSchema#string"/>
  </owl:DatatypeProperty>
</rdf:RDF>
