<?xml version="1.0" encoding="UTF-8"?>
<rdf:RDF
  xmlns:rdf="http://www.w3.org/1999/02/22-rdf-syntax-ns#"
  xmlns:rdfs="http://www.w3.org/2000/01/rdf-schema#"
  xmlns:owl="http://www.w3.org/2002/07/owl#"
  xmlns:xsd="http://www.w3.org/2001/XMLSchema#"
  xml:base="http://example.org/onto/">
  <owl:Class rdf:about="http://example.org/onto/class/google_apihub_host_project_registration">
    <rdfs:label>google_apihub_host_project_registration</rdfs:label>
    <rdfs:comment>#
#     ***     AUTO GENERATED CODE    ***    Type: MMv1     ***
#
# ----------------------------------------------------------------------------
#
#     This code is generated by Magic Modules using the following:
#
#     Configuration: https:#github.com/GoogleCloudPlatform/magic-modules/tree/main/mmv1/products/apihub/HostProjectRegistration.yaml
#     Template:      https:#github.com/GoogleCloudPlatform/magic-modules/tree/main/mmv1/templates/terraform/resource.html.markdown.tmpl
#
#     DO NOT EDIT this file directly. Any changes made to this file will be
#     overwritten during the next generation cycle.
#
# ----------------------------------------------------------------------------
subcategory: "API Hub"
description: |-
  Host project registration refers to the registration of a Google cloud project with API hub as a host project.
---</rdfs:comment>
  </owl:Class>
  <owl:DatatypeProperty rdf:about="http://example.org/onto/prop/google_apihub_host_project_registration_create_time">
    <rdfs:label>create_time</rdfs:label>
    <rdfs:comment>Output only. The time at which the host project registration was created.</rdfs:comment>
    <rdfs:domain rdf:resource="http://example.org/onto/class/google_apihub_host_project_registration"/>
    <rdfs:range rdf:resource="http://www.w3.org/2001/XMLSchema#string"/>
  </owl:DatatypeProperty>
  <owl:DatatypeProperty rdf:about="http://example.org/onto/prop/google_apihub_host_project_registration_gcp_project">
    <rdfs:label>gcp_project</rdfs:label>
    <rdfs:comment>Required. Immutable. Google cloud project name in the format: "projects/abc" or "projects/123".
As input, project name with either project id or number are accepted.
As output, this field will contain project number.</rdfs:comment>
    <rdfs:domain rdf:resource="http://example.org/onto/class/google_apihub_host_project_registration"/>
    <rdfs:range rdf:resource="http://www.w3.org/2001/XMLSchema#string"/>
  </owl:DatatypeProperty>
  <owl:DatatypeProperty rdf:about="http://example.org/onto/prop/google_apihub_host_project_registration_host_project_registration_id">
    <rdfs:label>host_project_registration_id</rdfs:label>
    <rdfs:comment>Required. The ID to use for the Host Project Registration, which will become the
final component of the host project registration's resource name. The ID
must be the same as the Google cloud project specified in the
host_project_registration.gcp_project field.</rdfs:comment>
    <rdfs:domain rdf:resource="http://example.org/onto/class/google_apihub_host_project_registration"/>
    <rdfs:range rdf:resource="http://www.w3.org/2001/XMLSchema#string"/>
  </owl:DatatypeProperty>
  <owl:DatatypeProperty rdf:about="http://example.org/onto/prop/google_apihub_host_project_registration_id">
    <rdfs:label>id</rdfs:label>
    <rdfs:domain rdf:resource="http://example.org/onto/class/google_apihub_host_project_registration"/>
    <rdfs:range rdf:resource="http://www.w3.org/2001/XMLSchema#string"/>
  </owl:DatatypeProperty>
  <owl:DatatypeProperty rdf:about="http://example.org/onto/prop/google_apihub_host_project_registration_location">
    <rdfs:label>location</rdfs:label>
    <rdfs:comment>Part of 'parent'. See documentation of 'projectsId'.</rdfs:comment>
    <rdfs:domain rdf:resource="http://example.org/onto/class/google_apihub_host_project_registration"/>
    <rdfs:range rdf:resource="http://www.w3.org/2001/XMLSchema#string"/>
  </owl:DatatypeProperty>
  <owl:DatatypeProperty rdf:about="http://example.org/onto/prop/google_apihub_host_project_registration_name">
    <rdfs:label>name</rdfs:label>
    <rdfs:comment>Identifier. The name of the host project registration.
Format:
"projects/{project}/locations/{location}/hostProjectRegistrations/{host_project_registration}".</rdfs:comment>
    <rdfs:domain rdf:resource="http://example.org/onto/class/google_apihub_host_project_registration"/>
    <rdfs:range rdf:resource="http://www.w3.org/2001/XMLSchema#string"/>
  </owl:DatatypeProperty>
  <owl:DatatypeProperty rdf:about="http://example.org/onto/prop/google_apihub_host_project_registration_project">
    <rdfs:label>project</rdfs:label>
    <rdfs:domain rdf:resource="http://example.org/onto/class/google_apihub_host_project_registration"/>
    <rdfs:range rdf:resource="http://www.w3.org/2001/XMLSchema#string"/>
  </owl:DatatypeProperty>
  <owl:DatatypeProperty rdf:about="http://example.org/onto/prop/google_apihub_host_project_registration_create">
    <rdfs:label>create</rdfs:label>
    <rdfs:domain rdf:resource="http://example.org/onto/class/google_apihub_host_project_registration"/>
    <rdfs:range rdf:resource="http://www.w3.org/2001/XMLSchema#string"/>
  </owl:DatatypeProperty>
  <owl:DatatypeProperty rdf:about="http://example.org/onto/prop/google_apihub_host_project_registration_delete">
    <rdfs:label>delete</rdfs:label>
    <rdfs:domain rdf:resource="http://example.org/onto/class/google_apihub_host_project_registration"/>
    <rdfs:range rdf:resource="http://www.w3.org/2001/XMLSchema#string"/>
  </owl:DatatypeProperty>
</rdf:RDF>
