<?xml version="1.0" encoding="UTF-8"?>
<rdf:RDF
  xmlns:rdf="http://www.w3.org/1999/02/22-rdf-syntax-ns#"
  xmlns:rdfs="http://www.w3.org/2000/01/rdf-schema#"
  xmlns:owl="http://www.w3.org/2002/07/owl#"
  xmlns:xsd="http://www.w3.org/2001/XMLSchema#"
  xml:base="http://example.org/onto/">
  <owl:Class rdf:about="http://example.org/onto/class/google_firebase_app_hosting_build">
    <rdfs:label>google_firebase_app_hosting_build</rdfs:label>
    <rdfs:comment>#
#     ***     AUTO GENERATED CODE    ***    Type: MMv1     ***
#
# ----------------------------------------------------------------------------
#
#     This code is generated by Magic Modules using the following:
#
#     Configuration: https:#github.com/GoogleCloudPlatform/magic-modules/tree/main/mmv1/products/firebaseapphosting/Build.yaml
#     Template:      https:#github.com/GoogleCloudPlatform/magic-modules/tree/main/mmv1/templates/terraform/resource.html.markdown.tmpl
#
#     DO NOT EDIT this file directly. Any changes made to this file will be
#     overwritten during the next generation cycle.
#
# ----------------------------------------------------------------------------
subcategory: "Firebase App Hosting"
description: |-
  A single build for a backend, at a specific point codebase reference tag
  and point in time.
---</rdfs:comment>
  </owl:Class>
  <owl:DatatypeProperty rdf:about="http://example.org/onto/prop/google_firebase_app_hosting_build_annotations">
    <rdfs:label>annotations</rdfs:label>
    <rdfs:comment>Unstructured key value map that may be set by external tools to
store and arbitrary metadata. They are not queryable and should be
preserved when modifying objects.

**Note**: This field is non-authoritative, and will only manage the annotations present in your configuration.
Please refer to the field 'effective_annotations' for all of the annotations present on the resource.</rdfs:comment>
    <rdfs:domain rdf:resource="http://example.org/onto/class/google_firebase_app_hosting_build"/>
    <rdfs:range rdf:resource="http://www.w3.org/2001/XMLSchema#string"/>
  </owl:DatatypeProperty>
  <owl:DatatypeProperty rdf:about="http://example.org/onto/prop/google_firebase_app_hosting_build_backend">
    <rdfs:label>backend</rdfs:label>
    <rdfs:comment>The ID of the Backend that this Build applies to</rdfs:comment>
    <rdfs:domain rdf:resource="http://example.org/onto/class/google_firebase_app_hosting_build"/>
    <rdfs:range rdf:resource="http://www.w3.org/2001/XMLSchema#string"/>
  </owl:DatatypeProperty>
  <owl:DatatypeProperty rdf:about="http://example.org/onto/prop/google_firebase_app_hosting_build_build_id">
    <rdfs:label>build_id</rdfs:label>
    <rdfs:comment>The user-specified ID of the build being created.</rdfs:comment>
    <rdfs:domain rdf:resource="http://example.org/onto/class/google_firebase_app_hosting_build"/>
    <rdfs:range rdf:resource="http://www.w3.org/2001/XMLSchema#string"/>
  </owl:DatatypeProperty>
  <owl:DatatypeProperty rdf:about="http://example.org/onto/prop/google_firebase_app_hosting_build_build_logs_uri">
    <rdfs:label>build_logs_uri</rdfs:label>
    <rdfs:comment>The location of the [Cloud Build
logs](https://cloud.google.com/build/docs/view-build-results) for the build
process.</rdfs:comment>
    <rdfs:domain rdf:resource="http://example.org/onto/class/google_firebase_app_hosting_build"/>
    <rdfs:range rdf:resource="http://www.w3.org/2001/XMLSchema#string"/>
  </owl:DatatypeProperty>
  <owl:DatatypeProperty rdf:about="http://example.org/onto/prop/google_firebase_app_hosting_build_create_time">
    <rdfs:label>create_time</rdfs:label>
    <rdfs:comment>Time at which the build was created.</rdfs:comment>
    <rdfs:domain rdf:resource="http://example.org/onto/class/google_firebase_app_hosting_build"/>
    <rdfs:range rdf:resource="http://www.w3.org/2001/XMLSchema#string"/>
  </owl:DatatypeProperty>
  <owl:DatatypeProperty rdf:about="http://example.org/onto/prop/google_firebase_app_hosting_build_display_name">
    <rdfs:label>display_name</rdfs:label>
    <rdfs:comment>Human-readable name. 63 character limit.</rdfs:comment>
    <rdfs:domain rdf:resource="http://example.org/onto/class/google_firebase_app_hosting_build"/>
    <rdfs:range rdf:resource="http://www.w3.org/2001/XMLSchema#string"/>
  </owl:DatatypeProperty>
  <owl:DatatypeProperty rdf:about="http://example.org/onto/prop/google_firebase_app_hosting_build_effective_annotations">
    <rdfs:label>effective_annotations</rdfs:label>
    <rdfs:comment>All of annotations (key/value pairs) present on the resource in GCP, including the annotations configured through Terraform, other clients and services.</rdfs:comment>
    <rdfs:domain rdf:resource="http://example.org/onto/class/google_firebase_app_hosting_build"/>
    <rdfs:range rdf:resource="http://www.w3.org/2001/XMLSchema#string"/>
  </owl:DatatypeProperty>
  <owl:DatatypeProperty rdf:about="http://example.org/onto/prop/google_firebase_app_hosting_build_effective_labels">
    <rdfs:label>effective_labels</rdfs:label>
    <rdfs:comment>All of labels (key/value pairs) present on the resource in GCP, including the labels configured through Terraform, other clients and services.</rdfs:comment>
    <rdfs:domain rdf:resource="http://example.org/onto/class/google_firebase_app_hosting_build"/>
    <rdfs:range rdf:resource="http://www.w3.org/2001/XMLSchema#string"/>
  </owl:DatatypeProperty>
  <owl:DatatypeProperty rdf:about="http://example.org/onto/prop/google_firebase_app_hosting_build_environment">
    <rdfs:label>environment</rdfs:label>
    <rdfs:comment>The environment name of the backend when this build was created.</rdfs:comment>
    <rdfs:domain rdf:resource="http://example.org/onto/class/google_firebase_app_hosting_build"/>
    <rdfs:range rdf:resource="http://www.w3.org/2001/XMLSchema#string"/>
  </owl:DatatypeProperty>
  <owl:DatatypeProperty rdf:about="http://example.org/onto/prop/google_firebase_app_hosting_build_error">
    <rdfs:label>error</rdfs:label>
    <rdfs:comment>The 'Status' type defines a logical error model that is suitable for
different programming environments, including REST APIs and RPC APIs. It is
used by [gRPC](https://github.com/grpc). Each 'Status' message contains
three pieces of data: error code, error message, and error details.

You can find out more about this error model and how to work with it in the
[API Design Guide](https://cloud.google.com/apis/design/errors).</rdfs:comment>
    <rdfs:domain rdf:resource="http://example.org/onto/class/google_firebase_app_hosting_build"/>
    <rdfs:range rdf:resource="http://www.w3.org/2001/XMLSchema#string"/>
  </owl:DatatypeProperty>
  <owl:DatatypeProperty rdf:about="http://example.org/onto/prop/google_firebase_app_hosting_build_error_source">
    <rdfs:label>error_source</rdfs:label>
    <rdfs:comment>The source of the error for the build, if in a 'FAILED' state.
Possible values:
CLOUD_BUILD
CLOUD_RUN</rdfs:comment>
    <rdfs:domain rdf:resource="http://example.org/onto/class/google_firebase_app_hosting_build"/>
    <rdfs:range rdf:resource="http://www.w3.org/2001/XMLSchema#string"/>
  </owl:DatatypeProperty>
  <owl:DatatypeProperty rdf:about="http://example.org/onto/prop/google_firebase_app_hosting_build_etag">
    <rdfs:label>etag</rdfs:label>
    <rdfs:comment>Server-computed checksum based on other values; may be sent
on update or delete to ensure operation is done on expected resource.</rdfs:comment>
    <rdfs:domain rdf:resource="http://example.org/onto/class/google_firebase_app_hosting_build"/>
    <rdfs:range rdf:resource="http://www.w3.org/2001/XMLSchema#string"/>
  </owl:DatatypeProperty>
  <owl:DatatypeProperty rdf:about="http://example.org/onto/prop/google_firebase_app_hosting_build_id">
    <rdfs:label>id</rdfs:label>
    <rdfs:domain rdf:resource="http://example.org/onto/class/google_firebase_app_hosting_build"/>
    <rdfs:range rdf:resource="http://www.w3.org/2001/XMLSchema#string"/>
  </owl:DatatypeProperty>
  <owl:DatatypeProperty rdf:about="http://example.org/onto/prop/google_firebase_app_hosting_build_image">
    <rdfs:label>image</rdfs:label>
    <rdfs:comment>The Artifact Registry
[container
image](https://cloud.google.com/artifact-registry/docs/reference/rest/v1/projects.locations.repositories.dockerImages)
URI, used by the Cloud Run
['revision'](https://cloud.google.com/run/docs/reference/rest/v2/projects.locations.services.revisions)
for this build.</rdfs:comment>
    <rdfs:domain rdf:resource="http://example.org/onto/class/google_firebase_app_hosting_build"/>
    <rdfs:range rdf:resource="http://www.w3.org/2001/XMLSchema#string"/>
  </owl:DatatypeProperty>
  <owl:DatatypeProperty rdf:about="http://example.org/onto/prop/google_firebase_app_hosting_build_labels">
    <rdfs:label>labels</rdfs:label>
    <rdfs:comment>Unstructured key value map that can be used to organize and categorize
objects.

**Note**: This field is non-authoritative, and will only manage the labels present in your configuration.
Please refer to the field 'effective_labels' for all of the labels present on the resource.</rdfs:comment>
    <rdfs:domain rdf:resource="http://example.org/onto/class/google_firebase_app_hosting_build"/>
    <rdfs:range rdf:resource="http://www.w3.org/2001/XMLSchema#string"/>
  </owl:DatatypeProperty>
  <owl:DatatypeProperty rdf:about="http://example.org/onto/prop/google_firebase_app_hosting_build_location">
    <rdfs:label>location</rdfs:label>
    <rdfs:comment>The location of the Backend that this Build applies to</rdfs:comment>
    <rdfs:domain rdf:resource="http://example.org/onto/class/google_firebase_app_hosting_build"/>
    <rdfs:range rdf:resource="http://www.w3.org/2001/XMLSchema#string"/>
  </owl:DatatypeProperty>
  <owl:DatatypeProperty rdf:about="http://example.org/onto/prop/google_firebase_app_hosting_build_name">
    <rdfs:label>name</rdfs:label>
    <rdfs:comment>Identifier. The resource name of the build.

Format:

'projects/{project}/locations/{locationId}/backends/{backendId}/builds/{buildId}'.</rdfs:comment>
    <rdfs:domain rdf:resource="http://example.org/onto/class/google_firebase_app_hosting_build"/>
    <rdfs:range rdf:resource="http://www.w3.org/2001/XMLSchema#string"/>
  </owl:DatatypeProperty>
  <owl:DatatypeProperty rdf:about="http://example.org/onto/prop/google_firebase_app_hosting_build_project">
    <rdfs:label>project</rdfs:label>
    <rdfs:domain rdf:resource="http://example.org/onto/class/google_firebase_app_hosting_build"/>
    <rdfs:range rdf:resource="http://www.w3.org/2001/XMLSchema#string"/>
  </owl:DatatypeProperty>
  <owl:DatatypeProperty rdf:about="http://example.org/onto/prop/google_firebase_app_hosting_build_state">
    <rdfs:label>state</rdfs:label>
    <rdfs:comment>The state of the build.
Possible values:
BUILDING
BUILT
DEPLOYING
READY
FAILED</rdfs:comment>
    <rdfs:domain rdf:resource="http://example.org/onto/class/google_firebase_app_hosting_build"/>
    <rdfs:range rdf:resource="http://www.w3.org/2001/XMLSchema#string"/>
  </owl:DatatypeProperty>
  <owl:DatatypeProperty rdf:about="http://example.org/onto/prop/google_firebase_app_hosting_build_terraform_labels">
    <rdfs:label>terraform_labels</rdfs:label>
    <rdfs:comment>The combination of labels configured directly on the resource
 and default labels configured on the provider.</rdfs:comment>
    <rdfs:domain rdf:resource="http://example.org/onto/class/google_firebase_app_hosting_build"/>
    <rdfs:range rdf:resource="http://www.w3.org/2001/XMLSchema#string"/>
  </owl:DatatypeProperty>
  <owl:DatatypeProperty rdf:about="http://example.org/onto/prop/google_firebase_app_hosting_build_uid">
    <rdfs:label>uid</rdfs:label>
    <rdfs:comment>System-assigned, unique identifier.</rdfs:comment>
    <rdfs:domain rdf:resource="http://example.org/onto/class/google_firebase_app_hosting_build"/>
    <rdfs:range rdf:resource="http://www.w3.org/2001/XMLSchema#string"/>
  </owl:DatatypeProperty>
  <owl:DatatypeProperty rdf:about="http://example.org/onto/prop/google_firebase_app_hosting_build_update_time">
    <rdfs:label>update_time</rdfs:label>
    <rdfs:comment>Time at which the build was last updated.</rdfs:comment>
    <rdfs:domain rdf:resource="http://example.org/onto/class/google_firebase_app_hosting_build"/>
    <rdfs:range rdf:resource="http://www.w3.org/2001/XMLSchema#string"/>
  </owl:DatatypeProperty>
  <owl:DatatypeProperty rdf:about="http://example.org/onto/prop/google_firebase_app_hosting_build_author">
    <rdfs:label>author</rdfs:label>
    <rdfs:comment>Version control metadata for a user associated with a resolved codebase.
Currently assumes a Git user.</rdfs:comment>
    <rdfs:domain rdf:resource="http://example.org/onto/class/google_firebase_app_hosting_build"/>
    <rdfs:range rdf:resource="http://www.w3.org/2001/XMLSchema#string"/>
  </owl:DatatypeProperty>
  <owl:DatatypeProperty rdf:about="http://example.org/onto/prop/google_firebase_app_hosting_build_branch">
    <rdfs:label>branch</rdfs:label>
    <rdfs:comment>The branch in the codebase to build from, using the latest commit.</rdfs:comment>
    <rdfs:domain rdf:resource="http://example.org/onto/class/google_firebase_app_hosting_build"/>
    <rdfs:range rdf:resource="http://www.w3.org/2001/XMLSchema#string"/>
  </owl:DatatypeProperty>
  <owl:DatatypeProperty rdf:about="http://example.org/onto/prop/google_firebase_app_hosting_build_commit">
    <rdfs:label>commit</rdfs:label>
    <rdfs:comment>The commit in the codebase to build from.</rdfs:comment>
    <rdfs:domain rdf:resource="http://example.org/onto/class/google_firebase_app_hosting_build"/>
    <rdfs:range rdf:resource="http://www.w3.org/2001/XMLSchema#string"/>
  </owl:DatatypeProperty>
  <owl:DatatypeProperty rdf:about="http://example.org/onto/prop/google_firebase_app_hosting_build_commit_message">
    <rdfs:label>commit_message</rdfs:label>
    <rdfs:comment>The message of a codebase change.</rdfs:comment>
    <rdfs:domain rdf:resource="http://example.org/onto/class/google_firebase_app_hosting_build"/>
    <rdfs:range rdf:resource="http://www.w3.org/2001/XMLSchema#string"/>
  </owl:DatatypeProperty>
  <owl:DatatypeProperty rdf:about="http://example.org/onto/prop/google_firebase_app_hosting_build_commit_time">
    <rdfs:label>commit_time</rdfs:label>
    <rdfs:comment>The time the change was made.</rdfs:comment>
    <rdfs:domain rdf:resource="http://example.org/onto/class/google_firebase_app_hosting_build"/>
    <rdfs:range rdf:resource="http://www.w3.org/2001/XMLSchema#string"/>
  </owl:DatatypeProperty>
  <owl:DatatypeProperty rdf:about="http://example.org/onto/prop/google_firebase_app_hosting_build_display_name">
    <rdfs:label>display_name</rdfs:label>
    <rdfs:comment>The human-friendly name to use for this Codebase when displaying a build.
We use the first eight characters of the SHA-1 hash for GitHub.com.</rdfs:comment>
    <rdfs:domain rdf:resource="http://example.org/onto/class/google_firebase_app_hosting_build"/>
    <rdfs:range rdf:resource="http://www.w3.org/2001/XMLSchema#string"/>
  </owl:DatatypeProperty>
  <owl:DatatypeProperty rdf:about="http://example.org/onto/prop/google_firebase_app_hosting_build_hash">
    <rdfs:label>hash</rdfs:label>
    <rdfs:comment>The full SHA-1 hash of a Git commit, if available.</rdfs:comment>
    <rdfs:domain rdf:resource="http://example.org/onto/class/google_firebase_app_hosting_build"/>
    <rdfs:range rdf:resource="http://www.w3.org/2001/XMLSchema#string"/>
  </owl:DatatypeProperty>
  <owl:DatatypeProperty rdf:about="http://example.org/onto/prop/google_firebase_app_hosting_build_uri">
    <rdfs:label>uri</rdfs:label>
    <rdfs:comment>A URI linking to the codebase on an hosting provider's website. May
not be valid if the commit has been rebased or force-pushed out of
existence in the linked repository.</rdfs:comment>
    <rdfs:domain rdf:resource="http://example.org/onto/class/google_firebase_app_hosting_build"/>
    <rdfs:range rdf:resource="http://www.w3.org/2001/XMLSchema#string"/>
  </owl:DatatypeProperty>
  <owl:DatatypeProperty rdf:about="http://example.org/onto/prop/google_firebase_app_hosting_build_image">
    <rdfs:label>image</rdfs:label>
    <rdfs:comment>A URI representing a container for the backend to use.</rdfs:comment>
    <rdfs:domain rdf:resource="http://example.org/onto/class/google_firebase_app_hosting_build"/>
    <rdfs:range rdf:resource="http://www.w3.org/2001/XMLSchema#string"/>
  </owl:DatatypeProperty>
  <owl:DatatypeProperty rdf:about="http://example.org/onto/prop/google_firebase_app_hosting_build_create">
    <rdfs:label>create</rdfs:label>
    <rdfs:domain rdf:resource="http://example.org/onto/class/google_firebase_app_hosting_build"/>
    <rdfs:range rdf:resource="http://www.w3.org/2001/XMLSchema#string"/>
  </owl:DatatypeProperty>
  <owl:DatatypeProperty rdf:about="http://example.org/onto/prop/google_firebase_app_hosting_build_delete">
    <rdfs:label>delete</rdfs:label>
    <rdfs:domain rdf:resource="http://example.org/onto/class/google_firebase_app_hosting_build"/>
    <rdfs:range rdf:resource="http://www.w3.org/2001/XMLSchema#string"/>
  </owl:DatatypeProperty>
  <owl:DatatypeProperty rdf:about="http://example.org/onto/prop/google_firebase_app_hosting_build_update">
    <rdfs:label>update</rdfs:label>
    <rdfs:domain rdf:resource="http://example.org/onto/class/google_firebase_app_hosting_build"/>
    <rdfs:range rdf:resource="http://www.w3.org/2001/XMLSchema#string"/>
  </owl:DatatypeProperty>
</rdf:RDF>
