<?xml version="1.0" encoding="UTF-8"?>
<rdf:RDF
  xmlns:rdf="http://www.w3.org/1999/02/22-rdf-syntax-ns#"
  xmlns:rdfs="http://www.w3.org/2000/01/rdf-schema#"
  xmlns:owl="http://www.w3.org/2002/07/owl#"
  xmlns:xsd="http://www.w3.org/2001/XMLSchema#"
  xml:base="http://example.org/onto/">
  <owl:Class rdf:about="http://example.org/onto/class/google_access_context_manager_gcp_user_access_binding">
    <rdfs:label>google_access_context_manager_gcp_user_access_binding</rdfs:label>
    <rdfs:comment>#
#     ***     AUTO GENERATED CODE    ***    Type: MMv1     ***
#
# ----------------------------------------------------------------------------
#
#     This code is generated by Magic Modules using the following:
#
#     Configuration: https:#github.com/GoogleCloudPlatform/magic-modules/tree/main/mmv1/products/accesscontextmanager/GcpUserAccessBinding.yaml
#     Template:      https:#github.com/GoogleCloudPlatform/magic-modules/tree/main/mmv1/templates/terraform/resource.html.markdown.tmpl
#
#     DO NOT EDIT this file directly. Any changes made to this file will be
#     overwritten during the next generation cycle.
#
# ----------------------------------------------------------------------------
subcategory: "Access Context Manager (VPC Service Controls)"
description: |-
  Restricts access to Cloud Console and Google Cloud APIs for a set of users using Context-Aware Access.
---</rdfs:comment>
  </owl:Class>
  <owl:DatatypeProperty rdf:about="http://example.org/onto/prop/google_access_context_manager_gcp_user_access_binding_access_levels">
    <rdfs:label>access_levels</rdfs:label>
    <rdfs:comment>Optional. Access level that a user must have to be granted access. Only one access level is supported, not multiple. This repeated field must have exactly one element. Example: "accessPolicies/9522/accessLevels/device_trusted"</rdfs:comment>
    <rdfs:domain rdf:resource="http://example.org/onto/class/google_access_context_manager_gcp_user_access_binding"/>
    <rdfs:range rdf:resource="http://www.w3.org/2001/XMLSchema#string"/>
  </owl:DatatypeProperty>
  <owl:DatatypeProperty rdf:about="http://example.org/onto/prop/google_access_context_manager_gcp_user_access_binding_group_key">
    <rdfs:label>group_key</rdfs:label>
    <rdfs:comment>Required. Immutable. Google Group id whose members are subject to this binding's restrictions. See "id" in the G Suite Directory API's Groups resource. If a group's email address/alias is changed, this resource will continue to point at the changed group. This field does not accept group email addresses or aliases. Example: "01d520gv4vjcrht"</rdfs:comment>
    <rdfs:domain rdf:resource="http://example.org/onto/class/google_access_context_manager_gcp_user_access_binding"/>
    <rdfs:range rdf:resource="http://www.w3.org/2001/XMLSchema#string"/>
  </owl:DatatypeProperty>
  <owl:DatatypeProperty rdf:about="http://example.org/onto/prop/google_access_context_manager_gcp_user_access_binding_id">
    <rdfs:label>id</rdfs:label>
    <rdfs:domain rdf:resource="http://example.org/onto/class/google_access_context_manager_gcp_user_access_binding"/>
    <rdfs:range rdf:resource="http://www.w3.org/2001/XMLSchema#string"/>
  </owl:DatatypeProperty>
  <owl:DatatypeProperty rdf:about="http://example.org/onto/prop/google_access_context_manager_gcp_user_access_binding_name">
    <rdfs:label>name</rdfs:label>
    <rdfs:comment>Immutable. Assigned by the server during creation. The last segment has an arbitrary length and has only URI unreserved characters (as defined by RFC 3986 Section 2.3). Should not be specified by the client during creation. Example: "organizations/256/gcpUserAccessBindings/b3-BhcX_Ud5N"</rdfs:comment>
    <rdfs:domain rdf:resource="http://example.org/onto/class/google_access_context_manager_gcp_user_access_binding"/>
    <rdfs:range rdf:resource="http://www.w3.org/2001/XMLSchema#string"/>
  </owl:DatatypeProperty>
  <owl:DatatypeProperty rdf:about="http://example.org/onto/prop/google_access_context_manager_gcp_user_access_binding_organization_id">
    <rdfs:label>organization_id</rdfs:label>
    <rdfs:comment>Required. ID of the parent organization.</rdfs:comment>
    <rdfs:domain rdf:resource="http://example.org/onto/class/google_access_context_manager_gcp_user_access_binding"/>
    <rdfs:range rdf:resource="http://www.w3.org/2001/XMLSchema#string"/>
  </owl:DatatypeProperty>
  <owl:DatatypeProperty rdf:about="http://example.org/onto/prop/google_access_context_manager_gcp_user_access_binding_access_levels">
    <rdfs:label>access_levels</rdfs:label>
    <rdfs:comment>Optional. Access level that a user must have to be granted access. Only one access level is supported, not multiple. This repeated field must have exactly one element. Example: "accessPolicies/9522/accessLevels/device_trusted"</rdfs:comment>
    <rdfs:domain rdf:resource="http://example.org/onto/class/google_access_context_manager_gcp_user_access_binding"/>
    <rdfs:range rdf:resource="http://www.w3.org/2001/XMLSchema#string"/>
  </owl:DatatypeProperty>
  <owl:DatatypeProperty rdf:about="http://example.org/onto/prop/google_access_context_manager_gcp_user_access_binding_max_inactivity">
    <rdfs:label>max_inactivity</rdfs:label>
    <rdfs:comment>Optional. How long a user is allowed to take between actions before a new access token must be issued. Only set for Google Cloud apps.</rdfs:comment>
    <rdfs:domain rdf:resource="http://example.org/onto/class/google_access_context_manager_gcp_user_access_binding"/>
    <rdfs:range rdf:resource="http://www.w3.org/2001/XMLSchema#string"/>
  </owl:DatatypeProperty>
  <owl:DatatypeProperty rdf:about="http://example.org/onto/prop/google_access_context_manager_gcp_user_access_binding_session_length">
    <rdfs:label>session_length</rdfs:label>
    <rdfs:comment>Optional. The session length. Setting this field to zero is equal to disabling session. Also can set infinite session by flipping the enabled bit to false below. If useOidcMaxAge is true, for OIDC apps, the session length will be the minimum of this field and OIDC max_age param.</rdfs:comment>
    <rdfs:domain rdf:resource="http://example.org/onto/class/google_access_context_manager_gcp_user_access_binding"/>
    <rdfs:range rdf:resource="http://www.w3.org/2001/XMLSchema#string"/>
  </owl:DatatypeProperty>
  <owl:DatatypeProperty rdf:about="http://example.org/onto/prop/google_access_context_manager_gcp_user_access_binding_session_length_enabled">
    <rdfs:label>session_length_enabled</rdfs:label>
    <rdfs:comment>Optional. This field enables or disables Google Cloud session length. When false, all fields set above will be disregarded and the session length is basically infinite.</rdfs:comment>
    <rdfs:domain rdf:resource="http://example.org/onto/class/google_access_context_manager_gcp_user_access_binding"/>
    <rdfs:range rdf:resource="http://www.w3.org/2001/XMLSchema#string"/>
  </owl:DatatypeProperty>
  <owl:DatatypeProperty rdf:about="http://example.org/onto/prop/google_access_context_manager_gcp_user_access_binding_session_reauth_method">
    <rdfs:label>session_reauth_method</rdfs:label>
    <rdfs:comment>Optional. The session challenges proposed to users when the Google Cloud session length is up. Possible values: ["LOGIN", "SECURITY_KEY", "PASSWORD"]</rdfs:comment>
    <rdfs:domain rdf:resource="http://example.org/onto/class/google_access_context_manager_gcp_user_access_binding"/>
    <rdfs:range rdf:resource="http://www.w3.org/2001/XMLSchema#string"/>
  </owl:DatatypeProperty>
  <owl:DatatypeProperty rdf:about="http://example.org/onto/prop/google_access_context_manager_gcp_user_access_binding_use_oidc_max_age">
    <rdfs:label>use_oidc_max_age</rdfs:label>
    <rdfs:comment>Optional. Only useful for OIDC apps. When false, the OIDC max_age param, if passed in the authentication request will be ignored. When true, the re-auth period will be the minimum of the sessionLength field and the max_age OIDC param.</rdfs:comment>
    <rdfs:domain rdf:resource="http://example.org/onto/class/google_access_context_manager_gcp_user_access_binding"/>
    <rdfs:range rdf:resource="http://www.w3.org/2001/XMLSchema#string"/>
  </owl:DatatypeProperty>
  <owl:DatatypeProperty rdf:about="http://example.org/onto/prop/google_access_context_manager_gcp_user_access_binding_access_levels">
    <rdfs:label>access_levels</rdfs:label>
    <rdfs:comment>Optional. Access level that a user must have to be granted access. Only one access level is supported, not multiple. This repeated field must have exactly one element. Example: "accessPolicies/9522/accessLevels/device_trusted"</rdfs:comment>
    <rdfs:domain rdf:resource="http://example.org/onto/class/google_access_context_manager_gcp_user_access_binding"/>
    <rdfs:range rdf:resource="http://www.w3.org/2001/XMLSchema#string"/>
  </owl:DatatypeProperty>
  <owl:DatatypeProperty rdf:about="http://example.org/onto/prop/google_access_context_manager_gcp_user_access_binding_client_id">
    <rdfs:label>client_id</rdfs:label>
    <rdfs:comment>The OAuth client ID of the application.</rdfs:comment>
    <rdfs:domain rdf:resource="http://example.org/onto/class/google_access_context_manager_gcp_user_access_binding"/>
    <rdfs:range rdf:resource="http://www.w3.org/2001/XMLSchema#string"/>
  </owl:DatatypeProperty>
  <owl:DatatypeProperty rdf:about="http://example.org/onto/prop/google_access_context_manager_gcp_user_access_binding_name">
    <rdfs:label>name</rdfs:label>
    <rdfs:comment>The name of the application. Example: "Cloud Console"</rdfs:comment>
    <rdfs:domain rdf:resource="http://example.org/onto/class/google_access_context_manager_gcp_user_access_binding"/>
    <rdfs:range rdf:resource="http://www.w3.org/2001/XMLSchema#string"/>
  </owl:DatatypeProperty>
  <owl:DatatypeProperty rdf:about="http://example.org/onto/prop/google_access_context_manager_gcp_user_access_binding_max_inactivity">
    <rdfs:label>max_inactivity</rdfs:label>
    <rdfs:comment>Optional. How long a user is allowed to take between actions before a new access token must be issued. Only set for Google Cloud apps.</rdfs:comment>
    <rdfs:domain rdf:resource="http://example.org/onto/class/google_access_context_manager_gcp_user_access_binding"/>
    <rdfs:range rdf:resource="http://www.w3.org/2001/XMLSchema#string"/>
  </owl:DatatypeProperty>
  <owl:DatatypeProperty rdf:about="http://example.org/onto/prop/google_access_context_manager_gcp_user_access_binding_session_length">
    <rdfs:label>session_length</rdfs:label>
    <rdfs:comment>Optional. The session length. Setting this field to zero is equal to disabling session. Also can set infinite session by flipping the enabled bit to false below. If useOidcMaxAge is true, for OIDC apps, the session length will be the minimum of this field and OIDC max_age param.</rdfs:comment>
    <rdfs:domain rdf:resource="http://example.org/onto/class/google_access_context_manager_gcp_user_access_binding"/>
    <rdfs:range rdf:resource="http://www.w3.org/2001/XMLSchema#string"/>
  </owl:DatatypeProperty>
  <owl:DatatypeProperty rdf:about="http://example.org/onto/prop/google_access_context_manager_gcp_user_access_binding_session_length_enabled">
    <rdfs:label>session_length_enabled</rdfs:label>
    <rdfs:comment>Optional. This field enables or disables Google Cloud session length. When false, all fields set above will be disregarded and the session length is basically infinite.</rdfs:comment>
    <rdfs:domain rdf:resource="http://example.org/onto/class/google_access_context_manager_gcp_user_access_binding"/>
    <rdfs:range rdf:resource="http://www.w3.org/2001/XMLSchema#string"/>
  </owl:DatatypeProperty>
  <owl:DatatypeProperty rdf:about="http://example.org/onto/prop/google_access_context_manager_gcp_user_access_binding_session_reauth_method">
    <rdfs:label>session_reauth_method</rdfs:label>
    <rdfs:comment>Optional. The session challenges proposed to users when the Google Cloud session length is up. Possible values: ["LOGIN", "SECURITY_KEY", "PASSWORD"]</rdfs:comment>
    <rdfs:domain rdf:resource="http://example.org/onto/class/google_access_context_manager_gcp_user_access_binding"/>
    <rdfs:range rdf:resource="http://www.w3.org/2001/XMLSchema#string"/>
  </owl:DatatypeProperty>
  <owl:DatatypeProperty rdf:about="http://example.org/onto/prop/google_access_context_manager_gcp_user_access_binding_use_oidc_max_age">
    <rdfs:label>use_oidc_max_age</rdfs:label>
    <rdfs:comment>Optional. Only useful for OIDC apps. When false, the OIDC max_age param, if passed in the authentication request will be ignored. When true, the re-auth period will be the minimum of the sessionLength field and the max_age OIDC param.</rdfs:comment>
    <rdfs:domain rdf:resource="http://example.org/onto/class/google_access_context_manager_gcp_user_access_binding"/>
    <rdfs:range rdf:resource="http://www.w3.org/2001/XMLSchema#string"/>
  </owl:DatatypeProperty>
  <owl:DatatypeProperty rdf:about="http://example.org/onto/prop/google_access_context_manager_gcp_user_access_binding_create">
    <rdfs:label>create</rdfs:label>
    <rdfs:domain rdf:resource="http://example.org/onto/class/google_access_context_manager_gcp_user_access_binding"/>
    <rdfs:range rdf:resource="http://www.w3.org/2001/XMLSchema#string"/>
  </owl:DatatypeProperty>
  <owl:DatatypeProperty rdf:about="http://example.org/onto/prop/google_access_context_manager_gcp_user_access_binding_delete">
    <rdfs:label>delete</rdfs:label>
    <rdfs:domain rdf:resource="http://example.org/onto/class/google_access_context_manager_gcp_user_access_binding"/>
    <rdfs:range rdf:resource="http://www.w3.org/2001/XMLSchema#string"/>
  </owl:DatatypeProperty>
  <owl:DatatypeProperty rdf:about="http://example.org/onto/prop/google_access_context_manager_gcp_user_access_binding_update">
    <rdfs:label>update</rdfs:label>
    <rdfs:domain rdf:resource="http://example.org/onto/class/google_access_context_manager_gcp_user_access_binding"/>
    <rdfs:range rdf:resource="http://www.w3.org/2001/XMLSchema#string"/>
  </owl:DatatypeProperty>
</rdf:RDF>
