<?xml version="1.0" encoding="UTF-8"?>
<rdf:RDF
  xmlns:rdf="http://www.w3.org/1999/02/22-rdf-syntax-ns#"
  xmlns:rdfs="http://www.w3.org/2000/01/rdf-schema#"
  xmlns:owl="http://www.w3.org/2002/07/owl#"
  xmlns:xsd="http://www.w3.org/2001/XMLSchema#"
  xml:base="http://example.org/onto/">
  <owl:Class rdf:about="http://example.org/onto/class/google_scc_v2_organization_scc_big_query_export">
    <rdfs:label>google_scc_v2_organization_scc_big_query_export</rdfs:label>
    <rdfs:comment>#
#     ***     AUTO GENERATED CODE    ***    Type: MMv1     ***
#
# ----------------------------------------------------------------------------
#
#     This code is generated by Magic Modules using the following:
#
#     Configuration: https:#github.com/GoogleCloudPlatform/magic-modules/tree/main/mmv1/products/securitycenterv2/OrganizationSccBigQueryExport.yaml
#     Template:      https:#github.com/GoogleCloudPlatform/magic-modules/tree/main/mmv1/templates/terraform/resource.html.markdown.tmpl
#
#     DO NOT EDIT this file directly. Any changes made to this file will be
#     overwritten during the next generation cycle.
#
# ----------------------------------------------------------------------------
subcategory: "Security Command Center (SCC) v2 API"
description: |-
  A Cloud Security Command Center (Cloud SCC) Big Query Export Config.
---</rdfs:comment>
  </owl:Class>
  <owl:DatatypeProperty rdf:about="http://example.org/onto/prop/google_scc_v2_organization_scc_big_query_export_big_query_export_id">
    <rdfs:label>big_query_export_id</rdfs:label>
    <rdfs:comment>This must be unique within the organization.</rdfs:comment>
    <rdfs:domain rdf:resource="http://example.org/onto/class/google_scc_v2_organization_scc_big_query_export"/>
    <rdfs:range rdf:resource="http://www.w3.org/2001/XMLSchema#string"/>
  </owl:DatatypeProperty>
  <owl:DatatypeProperty rdf:about="http://example.org/onto/prop/google_scc_v2_organization_scc_big_query_export_create_time">
    <rdfs:label>create_time</rdfs:label>
    <rdfs:comment>The time at which the BigQuery export was created. This field is set by the server and will be ignored if provided on export on creation.
A timestamp in RFC3339 UTC "Zulu" format, with nanosecond resolution and up to nine fractional digits.
Examples: "2014-10-02T15:01:23Z" and "2014-10-02T15:01:23.045123456Z".</rdfs:comment>
    <rdfs:domain rdf:resource="http://example.org/onto/class/google_scc_v2_organization_scc_big_query_export"/>
    <rdfs:range rdf:resource="http://www.w3.org/2001/XMLSchema#string"/>
  </owl:DatatypeProperty>
  <owl:DatatypeProperty rdf:about="http://example.org/onto/prop/google_scc_v2_organization_scc_big_query_export_dataset">
    <rdfs:label>dataset</rdfs:label>
    <rdfs:comment>The dataset to write findings' updates to.
Its format is "projects/[projectId]/datasets/[bigquery_dataset_id]".
BigQuery Dataset unique ID must contain only letters (a-z, A-Z), numbers (0-9), or underscores (_).</rdfs:comment>
    <rdfs:domain rdf:resource="http://example.org/onto/class/google_scc_v2_organization_scc_big_query_export"/>
    <rdfs:range rdf:resource="http://www.w3.org/2001/XMLSchema#string"/>
  </owl:DatatypeProperty>
  <owl:DatatypeProperty rdf:about="http://example.org/onto/prop/google_scc_v2_organization_scc_big_query_export_description">
    <rdfs:label>description</rdfs:label>
    <rdfs:comment>The description of the notification config (max of 1024 characters).</rdfs:comment>
    <rdfs:domain rdf:resource="http://example.org/onto/class/google_scc_v2_organization_scc_big_query_export"/>
    <rdfs:range rdf:resource="http://www.w3.org/2001/XMLSchema#string"/>
  </owl:DatatypeProperty>
  <owl:DatatypeProperty rdf:about="http://example.org/onto/prop/google_scc_v2_organization_scc_big_query_export_filter">
    <rdfs:label>filter</rdfs:label>
    <rdfs:comment>Expression that defines the filter to apply across create/update
events of findings. The
expression is a list of zero or more restrictions combined via
logical operators AND and OR. Parentheses are supported, and OR
has higher precedence than AND.

Restrictions have the form <field> <operator> <value> and may have
a - character in front of them to indicate negation. The fields
map to those defined in the corresponding resource.

The supported operators are:

* = for all value types.
* >, <, >=, <= for integer values.
* :, meaning substring matching, for strings.

The supported value types are:

* string literals in quotes.
* integer literals without quotes.
* boolean literals true and false without quotes.

See
[Filtering notifications](https://cloud.google.com/security-command-center/docs/how-to-api-filter-notifications)
for information on how to write a filter.</rdfs:comment>
    <rdfs:domain rdf:resource="http://example.org/onto/class/google_scc_v2_organization_scc_big_query_export"/>
    <rdfs:range rdf:resource="http://www.w3.org/2001/XMLSchema#string"/>
  </owl:DatatypeProperty>
  <owl:DatatypeProperty rdf:about="http://example.org/onto/prop/google_scc_v2_organization_scc_big_query_export_id">
    <rdfs:label>id</rdfs:label>
    <rdfs:domain rdf:resource="http://example.org/onto/class/google_scc_v2_organization_scc_big_query_export"/>
    <rdfs:range rdf:resource="http://www.w3.org/2001/XMLSchema#string"/>
  </owl:DatatypeProperty>
  <owl:DatatypeProperty rdf:about="http://example.org/onto/prop/google_scc_v2_organization_scc_big_query_export_location">
    <rdfs:label>location</rdfs:label>
    <rdfs:comment>location Id is provided by organization. If not provided, Use global as default.</rdfs:comment>
    <rdfs:domain rdf:resource="http://example.org/onto/class/google_scc_v2_organization_scc_big_query_export"/>
    <rdfs:range rdf:resource="http://www.w3.org/2001/XMLSchema#string"/>
  </owl:DatatypeProperty>
  <owl:DatatypeProperty rdf:about="http://example.org/onto/prop/google_scc_v2_organization_scc_big_query_export_most_recent_editor">
    <rdfs:label>most_recent_editor</rdfs:label>
    <rdfs:comment>Email address of the user who last edited the BigQuery export.
This field is set by the server and will be ignored if provided on export creation or update.</rdfs:comment>
    <rdfs:domain rdf:resource="http://example.org/onto/class/google_scc_v2_organization_scc_big_query_export"/>
    <rdfs:range rdf:resource="http://www.w3.org/2001/XMLSchema#string"/>
  </owl:DatatypeProperty>
  <owl:DatatypeProperty rdf:about="http://example.org/onto/prop/google_scc_v2_organization_scc_big_query_export_name">
    <rdfs:label>name</rdfs:label>
    <rdfs:comment>The resource name of this export, in the format
'organizations/{{organization}}/locations/{{location}}/bigQueryExports/{{big_query_export_id}}'.
This field is provided in responses, and is ignored when provided in create requests.</rdfs:comment>
    <rdfs:domain rdf:resource="http://example.org/onto/class/google_scc_v2_organization_scc_big_query_export"/>
    <rdfs:range rdf:resource="http://www.w3.org/2001/XMLSchema#string"/>
  </owl:DatatypeProperty>
  <owl:DatatypeProperty rdf:about="http://example.org/onto/prop/google_scc_v2_organization_scc_big_query_export_organization">
    <rdfs:label>organization</rdfs:label>
    <rdfs:comment>The organization whose Cloud Security Command Center the Big Query Export
Config lives in.</rdfs:comment>
    <rdfs:domain rdf:resource="http://example.org/onto/class/google_scc_v2_organization_scc_big_query_export"/>
    <rdfs:range rdf:resource="http://www.w3.org/2001/XMLSchema#string"/>
  </owl:DatatypeProperty>
  <owl:DatatypeProperty rdf:about="http://example.org/onto/prop/google_scc_v2_organization_scc_big_query_export_principal">
    <rdfs:label>principal</rdfs:label>
    <rdfs:comment>The service account that needs permission to create table and upload data to the BigQuery dataset.</rdfs:comment>
    <rdfs:domain rdf:resource="http://example.org/onto/class/google_scc_v2_organization_scc_big_query_export"/>
    <rdfs:range rdf:resource="http://www.w3.org/2001/XMLSchema#string"/>
  </owl:DatatypeProperty>
  <owl:DatatypeProperty rdf:about="http://example.org/onto/prop/google_scc_v2_organization_scc_big_query_export_update_time">
    <rdfs:label>update_time</rdfs:label>
    <rdfs:comment>The most recent time at which the BigQuery export was updated. This field is set by the server and will be ignored if provided on export creation or update.
A timestamp in RFC3339 UTC "Zulu" format, with nanosecond resolution and up to nine fractional digits.
Examples: "2014-10-02T15:01:23Z" and "2014-10-02T15:01:23.045123456Z".</rdfs:comment>
    <rdfs:domain rdf:resource="http://example.org/onto/class/google_scc_v2_organization_scc_big_query_export"/>
    <rdfs:range rdf:resource="http://www.w3.org/2001/XMLSchema#string"/>
  </owl:DatatypeProperty>
  <owl:DatatypeProperty rdf:about="http://example.org/onto/prop/google_scc_v2_organization_scc_big_query_export_create">
    <rdfs:label>create</rdfs:label>
    <rdfs:domain rdf:resource="http://example.org/onto/class/google_scc_v2_organization_scc_big_query_export"/>
    <rdfs:range rdf:resource="http://www.w3.org/2001/XMLSchema#string"/>
  </owl:DatatypeProperty>
  <owl:DatatypeProperty rdf:about="http://example.org/onto/prop/google_scc_v2_organization_scc_big_query_export_delete">
    <rdfs:label>delete</rdfs:label>
    <rdfs:domain rdf:resource="http://example.org/onto/class/google_scc_v2_organization_scc_big_query_export"/>
    <rdfs:range rdf:resource="http://www.w3.org/2001/XMLSchema#string"/>
  </owl:DatatypeProperty>
  <owl:DatatypeProperty rdf:about="http://example.org/onto/prop/google_scc_v2_organization_scc_big_query_export_update">
    <rdfs:label>update</rdfs:label>
    <rdfs:domain rdf:resource="http://example.org/onto/class/google_scc_v2_organization_scc_big_query_export"/>
    <rdfs:range rdf:resource="http://www.w3.org/2001/XMLSchema#string"/>
  </owl:DatatypeProperty>
</rdf:RDF>
