<?xml version="1.0" encoding="UTF-8"?>
<rdf:RDF
  xmlns:rdf="http://www.w3.org/1999/02/22-rdf-syntax-ns#"
  xmlns:rdfs="http://www.w3.org/2000/01/rdf-schema#"
  xmlns:owl="http://www.w3.org/2002/07/owl#"
  xmlns:xsd="http://www.w3.org/2001/XMLSchema#"
  xml:base="http://example.org/onto/">
  <owl:Class rdf:about="http://example.org/onto/class/google_compute_network">
    <rdfs:label>google_compute_network</rdfs:label>
    <rdfs:comment>#
#     ***     AUTO GENERATED CODE    ***    Type: MMv1     ***
#
# ----------------------------------------------------------------------------
#
#     This code is generated by Magic Modules using the following:
#
#     Configuration: https:#github.com/GoogleCloudPlatform/magic-modules/tree/main/mmv1/products/compute/Network.yaml
#     Template:      https:#github.com/GoogleCloudPlatform/magic-modules/tree/main/mmv1/templates/terraform/resource.html.markdown.tmpl
#
#     DO NOT EDIT this file directly. Any changes made to this file will be
#     overwritten during the next generation cycle.
#
# ----------------------------------------------------------------------------
subcategory: "Compute Engine"
description: |-
  Manages a VPC network or legacy network resource on GCP.
---</rdfs:comment>
  </owl:Class>
  <owl:DatatypeProperty rdf:about="http://example.org/onto/prop/google_compute_network_auto_create_subnetworks">
    <rdfs:label>auto_create_subnetworks</rdfs:label>
    <rdfs:comment>When set to 'true', the network is created in "auto subnet mode" and
it will create a subnet for each region automatically across the
'10.128.0.0/9' address range.

When set to 'false', the network is created in "custom subnet mode" so
the user can explicitly connect subnetwork resources.</rdfs:comment>
    <rdfs:domain rdf:resource="http://example.org/onto/class/google_compute_network"/>
    <rdfs:range rdf:resource="http://www.w3.org/2001/XMLSchema#string"/>
  </owl:DatatypeProperty>
  <owl:DatatypeProperty rdf:about="http://example.org/onto/prop/google_compute_network_bgp_always_compare_med">
    <rdfs:label>bgp_always_compare_med</rdfs:label>
    <rdfs:comment>Enables/disables the comparison of MED across routes with different Neighbor ASNs.
This value can only be set if the --bgp-best-path-selection-mode is STANDARD</rdfs:comment>
    <rdfs:domain rdf:resource="http://example.org/onto/class/google_compute_network"/>
    <rdfs:range rdf:resource="http://www.w3.org/2001/XMLSchema#string"/>
  </owl:DatatypeProperty>
  <owl:DatatypeProperty rdf:about="http://example.org/onto/prop/google_compute_network_bgp_best_path_selection_mode">
    <rdfs:label>bgp_best_path_selection_mode</rdfs:label>
    <rdfs:comment>The BGP best selection algorithm to be employed. MODE can be LEGACY or STANDARD. Possible values: ["LEGACY", "STANDARD"]</rdfs:comment>
    <rdfs:domain rdf:resource="http://example.org/onto/class/google_compute_network"/>
    <rdfs:range rdf:resource="http://www.w3.org/2001/XMLSchema#string"/>
  </owl:DatatypeProperty>
  <owl:DatatypeProperty rdf:about="http://example.org/onto/prop/google_compute_network_bgp_inter_region_cost">
    <rdfs:label>bgp_inter_region_cost</rdfs:label>
    <rdfs:comment>Choice of the behavior of inter-regional cost and MED in the BPS algorithm. Possible values: ["DEFAULT", "ADD_COST_TO_MED"]</rdfs:comment>
    <rdfs:domain rdf:resource="http://example.org/onto/class/google_compute_network"/>
    <rdfs:range rdf:resource="http://www.w3.org/2001/XMLSchema#string"/>
  </owl:DatatypeProperty>
  <owl:DatatypeProperty rdf:about="http://example.org/onto/prop/google_compute_network_delete_default_routes_on_create">
    <rdfs:label>delete_default_routes_on_create</rdfs:label>
    <rdfs:comment>If set to 'true', default routes ('0.0.0.0/0') will be deleted
immediately after network creation. Defaults to 'false'.</rdfs:comment>
    <rdfs:domain rdf:resource="http://example.org/onto/class/google_compute_network"/>
    <rdfs:range rdf:resource="http://www.w3.org/2001/XMLSchema#string"/>
  </owl:DatatypeProperty>
  <owl:DatatypeProperty rdf:about="http://example.org/onto/prop/google_compute_network_description">
    <rdfs:label>description</rdfs:label>
    <rdfs:comment>An optional description of this resource. The resource must be
recreated to modify this field.</rdfs:comment>
    <rdfs:domain rdf:resource="http://example.org/onto/class/google_compute_network"/>
    <rdfs:range rdf:resource="http://www.w3.org/2001/XMLSchema#string"/>
  </owl:DatatypeProperty>
  <owl:DatatypeProperty rdf:about="http://example.org/onto/prop/google_compute_network_enable_ula_internal_ipv6">
    <rdfs:label>enable_ula_internal_ipv6</rdfs:label>
    <rdfs:comment>Enable ULA internal ipv6 on this network. Enabling this feature will assign
a /48 from google defined ULA prefix fd20::/20.</rdfs:comment>
    <rdfs:domain rdf:resource="http://example.org/onto/class/google_compute_network"/>
    <rdfs:range rdf:resource="http://www.w3.org/2001/XMLSchema#string"/>
  </owl:DatatypeProperty>
  <owl:DatatypeProperty rdf:about="http://example.org/onto/prop/google_compute_network_gateway_ipv4">
    <rdfs:label>gateway_ipv4</rdfs:label>
    <rdfs:comment>The gateway address for default routing out of the network. This value
is selected by GCP.</rdfs:comment>
    <rdfs:domain rdf:resource="http://example.org/onto/class/google_compute_network"/>
    <rdfs:range rdf:resource="http://www.w3.org/2001/XMLSchema#string"/>
  </owl:DatatypeProperty>
  <owl:DatatypeProperty rdf:about="http://example.org/onto/prop/google_compute_network_id">
    <rdfs:label>id</rdfs:label>
    <rdfs:domain rdf:resource="http://example.org/onto/class/google_compute_network"/>
    <rdfs:range rdf:resource="http://www.w3.org/2001/XMLSchema#string"/>
  </owl:DatatypeProperty>
  <owl:DatatypeProperty rdf:about="http://example.org/onto/prop/google_compute_network_internal_ipv6_range">
    <rdfs:label>internal_ipv6_range</rdfs:label>
    <rdfs:comment>When enabling ula internal ipv6, caller optionally can specify the /48 range
they want from the google defined ULA prefix fd20::/20. The input must be a
valid /48 ULA IPv6 address and must be within the fd20::/20. Operation will
fail if the speficied /48 is already in used by another resource.
If the field is not speficied, then a /48 range will be randomly allocated from fd20::/20 and returned via this field.</rdfs:comment>
    <rdfs:domain rdf:resource="http://example.org/onto/class/google_compute_network"/>
    <rdfs:range rdf:resource="http://www.w3.org/2001/XMLSchema#string"/>
  </owl:DatatypeProperty>
  <owl:DatatypeProperty rdf:about="http://example.org/onto/prop/google_compute_network_mtu">
    <rdfs:label>mtu</rdfs:label>
    <rdfs:comment>Maximum Transmission Unit in bytes. The default value is 1460 bytes.
The minimum value for this field is 1300 and the maximum value is 8896 bytes (jumbo frames).
Note that packets larger than 1500 bytes (standard Ethernet) can be subject to TCP-MSS clamping or dropped
with an ICMP 'Fragmentation-Needed' message if the packets are routed to the Internet or other VPCs
with varying MTUs.</rdfs:comment>
    <rdfs:domain rdf:resource="http://example.org/onto/class/google_compute_network"/>
    <rdfs:range rdf:resource="http://www.w3.org/2001/XMLSchema#string"/>
  </owl:DatatypeProperty>
  <owl:DatatypeProperty rdf:about="http://example.org/onto/prop/google_compute_network_name">
    <rdfs:label>name</rdfs:label>
    <rdfs:comment>Name of the resource. Provided by the client when the resource is
created. The name must be 1-63 characters long, and comply with
RFC1035. Specifically, the name must be 1-63 characters long and match
the regular expression '[a-z]([-a-z0-9]*[a-z0-9])?' which means the
first character must be a lowercase letter, and all following
characters must be a dash, lowercase letter, or digit, except the last
character, which cannot be a dash.</rdfs:comment>
    <rdfs:domain rdf:resource="http://example.org/onto/class/google_compute_network"/>
    <rdfs:range rdf:resource="http://www.w3.org/2001/XMLSchema#string"/>
  </owl:DatatypeProperty>
  <owl:DatatypeProperty rdf:about="http://example.org/onto/prop/google_compute_network_network_firewall_policy_enforcement_order">
    <rdfs:label>network_firewall_policy_enforcement_order</rdfs:label>
    <rdfs:comment>Set the order that Firewall Rules and Firewall Policies are evaluated. Default value: "AFTER_CLASSIC_FIREWALL" Possible values: ["BEFORE_CLASSIC_FIREWALL", "AFTER_CLASSIC_FIREWALL"]</rdfs:comment>
    <rdfs:domain rdf:resource="http://example.org/onto/class/google_compute_network"/>
    <rdfs:range rdf:resource="http://www.w3.org/2001/XMLSchema#string"/>
  </owl:DatatypeProperty>
  <owl:DatatypeProperty rdf:about="http://example.org/onto/prop/google_compute_network_network_id">
    <rdfs:label>network_id</rdfs:label>
    <rdfs:comment>The unique identifier for the resource. This identifier is defined by the server.</rdfs:comment>
    <rdfs:domain rdf:resource="http://example.org/onto/class/google_compute_network"/>
    <rdfs:range rdf:resource="http://www.w3.org/2001/XMLSchema#string"/>
  </owl:DatatypeProperty>
  <owl:DatatypeProperty rdf:about="http://example.org/onto/prop/google_compute_network_network_profile">
    <rdfs:label>network_profile</rdfs:label>
    <rdfs:comment>A full or partial URL of the network profile to apply to this network.
This field can be set only at resource creation time. For example, the
following are valid URLs:
* https://www.googleapis.com/compute/v1/projects/{projectId}/global/networkProfiles/{network_profile_name}
* projects/{projectId}/global/networkProfiles/{network_profile_name}</rdfs:comment>
    <rdfs:domain rdf:resource="http://example.org/onto/class/google_compute_network"/>
    <rdfs:range rdf:resource="http://www.w3.org/2001/XMLSchema#string"/>
  </owl:DatatypeProperty>
  <owl:DatatypeProperty rdf:about="http://example.org/onto/prop/google_compute_network_numeric_id">
    <rdfs:label>numeric_id</rdfs:label>
    <rdfs:comment>The unique identifier for the resource. This identifier is defined by the server.</rdfs:comment>
    <rdfs:domain rdf:resource="http://example.org/onto/class/google_compute_network"/>
    <rdfs:range rdf:resource="http://www.w3.org/2001/XMLSchema#string"/>
  </owl:DatatypeProperty>
  <owl:DatatypeProperty rdf:about="http://example.org/onto/prop/google_compute_network_project">
    <rdfs:label>project</rdfs:label>
    <rdfs:domain rdf:resource="http://example.org/onto/class/google_compute_network"/>
    <rdfs:range rdf:resource="http://www.w3.org/2001/XMLSchema#string"/>
  </owl:DatatypeProperty>
  <owl:DatatypeProperty rdf:about="http://example.org/onto/prop/google_compute_network_routing_mode">
    <rdfs:label>routing_mode</rdfs:label>
    <rdfs:comment>The network-wide routing mode to use. If set to 'REGIONAL', this
network's cloud routers will only advertise routes with subnetworks
of this network in the same region as the router. If set to 'GLOBAL',
this network's cloud routers will advertise routes with all
subnetworks of this network, across regions. Possible values: ["REGIONAL", "GLOBAL"]</rdfs:comment>
    <rdfs:domain rdf:resource="http://example.org/onto/class/google_compute_network"/>
    <rdfs:range rdf:resource="http://www.w3.org/2001/XMLSchema#string"/>
  </owl:DatatypeProperty>
  <owl:DatatypeProperty rdf:about="http://example.org/onto/prop/google_compute_network_self_link">
    <rdfs:label>self_link</rdfs:label>
    <rdfs:domain rdf:resource="http://example.org/onto/class/google_compute_network"/>
    <rdfs:range rdf:resource="http://www.w3.org/2001/XMLSchema#string"/>
  </owl:DatatypeProperty>
  <owl:DatatypeProperty rdf:about="http://example.org/onto/prop/google_compute_network_resource_manager_tags">
    <rdfs:label>resource_manager_tags</rdfs:label>
    <rdfs:comment>Resource manager tags to be bound to the network. Tag keys and values have the
same definition as resource manager tags. Keys must be in the format tagKeys/{tag_key_id},
and values are in the format tagValues/456.</rdfs:comment>
    <rdfs:domain rdf:resource="http://example.org/onto/class/google_compute_network"/>
    <rdfs:range rdf:resource="http://www.w3.org/2001/XMLSchema#string"/>
  </owl:DatatypeProperty>
  <owl:DatatypeProperty rdf:about="http://example.org/onto/prop/google_compute_network_create">
    <rdfs:label>create</rdfs:label>
    <rdfs:domain rdf:resource="http://example.org/onto/class/google_compute_network"/>
    <rdfs:range rdf:resource="http://www.w3.org/2001/XMLSchema#string"/>
  </owl:DatatypeProperty>
  <owl:DatatypeProperty rdf:about="http://example.org/onto/prop/google_compute_network_delete">
    <rdfs:label>delete</rdfs:label>
    <rdfs:domain rdf:resource="http://example.org/onto/class/google_compute_network"/>
    <rdfs:range rdf:resource="http://www.w3.org/2001/XMLSchema#string"/>
  </owl:DatatypeProperty>
  <owl:DatatypeProperty rdf:about="http://example.org/onto/prop/google_compute_network_update">
    <rdfs:label>update</rdfs:label>
    <rdfs:domain rdf:resource="http://example.org/onto/class/google_compute_network"/>
    <rdfs:range rdf:resource="http://www.w3.org/2001/XMLSchema#string"/>
  </owl:DatatypeProperty>
</rdf:RDF>
