<?xml version="1.0" encoding="UTF-8"?>
<rdf:RDF
  xmlns:rdf="http://www.w3.org/1999/02/22-rdf-syntax-ns#"
  xmlns:rdfs="http://www.w3.org/2000/01/rdf-schema#"
  xmlns:owl="http://www.w3.org/2002/07/owl#"
  xmlns:xsd="http://www.w3.org/2001/XMLSchema#"
  xml:base="http://example.org/onto/">
  <owl:Class rdf:about="http://example.org/onto/class/google_compute_region_network_endpoint_group">
    <rdfs:label>google_compute_region_network_endpoint_group</rdfs:label>
    <rdfs:comment>#
#     ***     AUTO GENERATED CODE    ***    Type: MMv1     ***
#
# ----------------------------------------------------------------------------
#
#     This code is generated by Magic Modules using the following:
#
#     Configuration: https:#github.com/GoogleCloudPlatform/magic-modules/tree/main/mmv1/products/compute/RegionNetworkEndpointGroup.yaml
#     Template:      https:#github.com/GoogleCloudPlatform/magic-modules/tree/main/mmv1/templates/terraform/resource.html.markdown.tmpl
#
#     DO NOT EDIT this file directly. Any changes made to this file will be
#     overwritten during the next generation cycle.
#
# ----------------------------------------------------------------------------
subcategory: "Compute Engine"
description: |-
  A regional NEG that can support Serverless Products, proxying traffic to
  external backends and providing traffic to the PSC port mapping endpoints.
---</rdfs:comment>
  </owl:Class>
  <owl:DatatypeProperty rdf:about="http://example.org/onto/prop/google_compute_region_network_endpoint_group_description">
    <rdfs:label>description</rdfs:label>
    <rdfs:comment>An optional description of this resource. Provide this property when
you create the resource.</rdfs:comment>
    <rdfs:domain rdf:resource="http://example.org/onto/class/google_compute_region_network_endpoint_group"/>
    <rdfs:range rdf:resource="http://www.w3.org/2001/XMLSchema#string"/>
  </owl:DatatypeProperty>
  <owl:DatatypeProperty rdf:about="http://example.org/onto/prop/google_compute_region_network_endpoint_group_id">
    <rdfs:label>id</rdfs:label>
    <rdfs:domain rdf:resource="http://example.org/onto/class/google_compute_region_network_endpoint_group"/>
    <rdfs:range rdf:resource="http://www.w3.org/2001/XMLSchema#string"/>
  </owl:DatatypeProperty>
  <owl:DatatypeProperty rdf:about="http://example.org/onto/prop/google_compute_region_network_endpoint_group_name">
    <rdfs:label>name</rdfs:label>
    <rdfs:comment>Name of the resource; provided by the client when the resource is
created. The name must be 1-63 characters long, and comply with
RFC1035. Specifically, the name must be 1-63 characters long and match
the regular expression '[a-z]([-a-z0-9]*[a-z0-9])?' which means the
first character must be a lowercase letter, and all following
characters must be a dash, lowercase letter, or digit, except the last
character, which cannot be a dash.</rdfs:comment>
    <rdfs:domain rdf:resource="http://example.org/onto/class/google_compute_region_network_endpoint_group"/>
    <rdfs:range rdf:resource="http://www.w3.org/2001/XMLSchema#string"/>
  </owl:DatatypeProperty>
  <owl:DatatypeProperty rdf:about="http://example.org/onto/prop/google_compute_region_network_endpoint_group_network">
    <rdfs:label>network</rdfs:label>
    <rdfs:comment>This field is only used for PSC and INTERNET NEGs.

The URL of the network to which all network endpoints in the NEG belong. Uses
"default" project network if unspecified.</rdfs:comment>
    <rdfs:domain rdf:resource="http://example.org/onto/class/google_compute_region_network_endpoint_group"/>
    <rdfs:range rdf:resource="http://www.w3.org/2001/XMLSchema#string"/>
  </owl:DatatypeProperty>
  <owl:DatatypeProperty rdf:about="http://example.org/onto/prop/google_compute_region_network_endpoint_group_network_endpoint_type">
    <rdfs:label>network_endpoint_type</rdfs:label>
    <rdfs:comment>Type of network endpoints in this network endpoint group. Defaults to SERVERLESS. Default value: "SERVERLESS" Possible values: ["SERVERLESS", "PRIVATE_SERVICE_CONNECT", "INTERNET_IP_PORT", "INTERNET_FQDN_PORT", "GCE_VM_IP_PORTMAP"]</rdfs:comment>
    <rdfs:domain rdf:resource="http://example.org/onto/class/google_compute_region_network_endpoint_group"/>
    <rdfs:range rdf:resource="http://www.w3.org/2001/XMLSchema#string"/>
  </owl:DatatypeProperty>
  <owl:DatatypeProperty rdf:about="http://example.org/onto/prop/google_compute_region_network_endpoint_group_project">
    <rdfs:label>project</rdfs:label>
    <rdfs:domain rdf:resource="http://example.org/onto/class/google_compute_region_network_endpoint_group"/>
    <rdfs:range rdf:resource="http://www.w3.org/2001/XMLSchema#string"/>
  </owl:DatatypeProperty>
  <owl:DatatypeProperty rdf:about="http://example.org/onto/prop/google_compute_region_network_endpoint_group_psc_target_service">
    <rdfs:label>psc_target_service</rdfs:label>
    <rdfs:comment>This field is only used for PSC and INTERNET NEGs.

The target service url used to set up private service connection to
a Google API or a PSC Producer Service Attachment.</rdfs:comment>
    <rdfs:domain rdf:resource="http://example.org/onto/class/google_compute_region_network_endpoint_group"/>
    <rdfs:range rdf:resource="http://www.w3.org/2001/XMLSchema#string"/>
  </owl:DatatypeProperty>
  <owl:DatatypeProperty rdf:about="http://example.org/onto/prop/google_compute_region_network_endpoint_group_region">
    <rdfs:label>region</rdfs:label>
    <rdfs:comment>A reference to the region where the regional NEGs reside.</rdfs:comment>
    <rdfs:domain rdf:resource="http://example.org/onto/class/google_compute_region_network_endpoint_group"/>
    <rdfs:range rdf:resource="http://www.w3.org/2001/XMLSchema#string"/>
  </owl:DatatypeProperty>
  <owl:DatatypeProperty rdf:about="http://example.org/onto/prop/google_compute_region_network_endpoint_group_self_link">
    <rdfs:label>self_link</rdfs:label>
    <rdfs:domain rdf:resource="http://example.org/onto/class/google_compute_region_network_endpoint_group"/>
    <rdfs:range rdf:resource="http://www.w3.org/2001/XMLSchema#string"/>
  </owl:DatatypeProperty>
  <owl:DatatypeProperty rdf:about="http://example.org/onto/prop/google_compute_region_network_endpoint_group_subnetwork">
    <rdfs:label>subnetwork</rdfs:label>
    <rdfs:comment>This field is only used for PSC NEGs.

Optional URL of the subnetwork to which all network endpoints in the NEG belong.</rdfs:comment>
    <rdfs:domain rdf:resource="http://example.org/onto/class/google_compute_region_network_endpoint_group"/>
    <rdfs:range rdf:resource="http://www.w3.org/2001/XMLSchema#string"/>
  </owl:DatatypeProperty>
  <owl:DatatypeProperty rdf:about="http://example.org/onto/prop/google_compute_region_network_endpoint_group_service">
    <rdfs:label>service</rdfs:label>
    <rdfs:comment>Optional serving service.
The service name must be 1-63 characters long, and comply with RFC1035.
Example value: "default", "my-service".</rdfs:comment>
    <rdfs:domain rdf:resource="http://example.org/onto/class/google_compute_region_network_endpoint_group"/>
    <rdfs:range rdf:resource="http://www.w3.org/2001/XMLSchema#string"/>
  </owl:DatatypeProperty>
  <owl:DatatypeProperty rdf:about="http://example.org/onto/prop/google_compute_region_network_endpoint_group_url_mask">
    <rdfs:label>url_mask</rdfs:label>
    <rdfs:comment>A template to parse service and version fields from a request URL.
URL mask allows for routing to multiple App Engine services without
having to create multiple Network Endpoint Groups and backend services.

For example, the request URLs "foo1-dot-appname.appspot.com/v1" and
"foo1-dot-appname.appspot.com/v2" can be backed by the same Serverless NEG with
URL mask "-dot-appname.appspot.com/". The URL mask will parse
them to { service = "foo1", version = "v1" } and { service = "foo1", version = "v2" } respectively.</rdfs:comment>
    <rdfs:domain rdf:resource="http://example.org/onto/class/google_compute_region_network_endpoint_group"/>
    <rdfs:range rdf:resource="http://www.w3.org/2001/XMLSchema#string"/>
  </owl:DatatypeProperty>
  <owl:DatatypeProperty rdf:about="http://example.org/onto/prop/google_compute_region_network_endpoint_group_version">
    <rdfs:label>version</rdfs:label>
    <rdfs:comment>Optional serving version.
The version must be 1-63 characters long, and comply with RFC1035.
Example value: "v1", "v2".</rdfs:comment>
    <rdfs:domain rdf:resource="http://example.org/onto/class/google_compute_region_network_endpoint_group"/>
    <rdfs:range rdf:resource="http://www.w3.org/2001/XMLSchema#string"/>
  </owl:DatatypeProperty>
  <owl:DatatypeProperty rdf:about="http://example.org/onto/prop/google_compute_region_network_endpoint_group_function">
    <rdfs:label>function</rdfs:label>
    <rdfs:comment>A user-defined name of the Cloud Function.
The function name is case-sensitive and must be 1-63 characters long.
Example value: "func1".</rdfs:comment>
    <rdfs:domain rdf:resource="http://example.org/onto/class/google_compute_region_network_endpoint_group"/>
    <rdfs:range rdf:resource="http://www.w3.org/2001/XMLSchema#string"/>
  </owl:DatatypeProperty>
  <owl:DatatypeProperty rdf:about="http://example.org/onto/prop/google_compute_region_network_endpoint_group_url_mask">
    <rdfs:label>url_mask</rdfs:label>
    <rdfs:comment>A template to parse function field from a request URL. URL mask allows
for routing to multiple Cloud Functions without having to create
multiple Network Endpoint Groups and backend services.

For example, request URLs "mydomain.com/function1" and "mydomain.com/function2"
can be backed by the same Serverless NEG with URL mask "/". The URL mask
will parse them to { function = "function1" } and { function = "function2" } respectively.</rdfs:comment>
    <rdfs:domain rdf:resource="http://example.org/onto/class/google_compute_region_network_endpoint_group"/>
    <rdfs:range rdf:resource="http://www.w3.org/2001/XMLSchema#string"/>
  </owl:DatatypeProperty>
  <owl:DatatypeProperty rdf:about="http://example.org/onto/prop/google_compute_region_network_endpoint_group_service">
    <rdfs:label>service</rdfs:label>
    <rdfs:comment>Cloud Run service is the main resource of Cloud Run.
The service must be 1-63 characters long, and comply with RFC1035.
Example value: "run-service".</rdfs:comment>
    <rdfs:domain rdf:resource="http://example.org/onto/class/google_compute_region_network_endpoint_group"/>
    <rdfs:range rdf:resource="http://www.w3.org/2001/XMLSchema#string"/>
  </owl:DatatypeProperty>
  <owl:DatatypeProperty rdf:about="http://example.org/onto/prop/google_compute_region_network_endpoint_group_tag">
    <rdfs:label>tag</rdfs:label>
    <rdfs:comment>Cloud Run tag represents the "named-revision" to provide
additional fine-grained traffic routing information.
The tag must be 1-63 characters long, and comply with RFC1035.
Example value: "revision-0010".</rdfs:comment>
    <rdfs:domain rdf:resource="http://example.org/onto/class/google_compute_region_network_endpoint_group"/>
    <rdfs:range rdf:resource="http://www.w3.org/2001/XMLSchema#string"/>
  </owl:DatatypeProperty>
  <owl:DatatypeProperty rdf:about="http://example.org/onto/prop/google_compute_region_network_endpoint_group_url_mask">
    <rdfs:label>url_mask</rdfs:label>
    <rdfs:comment>A template to parse service and tag fields from a request URL.
URL mask allows for routing to multiple Run services without having
to create multiple network endpoint groups and backend services.

For example, request URLs "foo1.domain.com/bar1" and "foo1.domain.com/bar2"
an be backed by the same Serverless Network Endpoint Group (NEG) with
URL mask ".domain.com/". The URL mask will parse them to { service="bar1", tag="foo1" }
and { service="bar2", tag="foo2" } respectively.</rdfs:comment>
    <rdfs:domain rdf:resource="http://example.org/onto/class/google_compute_region_network_endpoint_group"/>
    <rdfs:range rdf:resource="http://www.w3.org/2001/XMLSchema#string"/>
  </owl:DatatypeProperty>
  <owl:DatatypeProperty rdf:about="http://example.org/onto/prop/google_compute_region_network_endpoint_group_producer_port">
    <rdfs:label>producer_port</rdfs:label>
    <rdfs:comment>The PSC producer port to use when consumer PSC NEG connects to a producer. If
this flag isn't specified for a PSC NEG with endpoint type
private-service-connect, then PSC NEG will be connected to a first port in the
available PSC producer port range.</rdfs:comment>
    <rdfs:domain rdf:resource="http://example.org/onto/class/google_compute_region_network_endpoint_group"/>
    <rdfs:range rdf:resource="http://www.w3.org/2001/XMLSchema#string"/>
  </owl:DatatypeProperty>
  <owl:DatatypeProperty rdf:about="http://example.org/onto/prop/google_compute_region_network_endpoint_group_create">
    <rdfs:label>create</rdfs:label>
    <rdfs:domain rdf:resource="http://example.org/onto/class/google_compute_region_network_endpoint_group"/>
    <rdfs:range rdf:resource="http://www.w3.org/2001/XMLSchema#string"/>
  </owl:DatatypeProperty>
  <owl:DatatypeProperty rdf:about="http://example.org/onto/prop/google_compute_region_network_endpoint_group_delete">
    <rdfs:label>delete</rdfs:label>
    <rdfs:domain rdf:resource="http://example.org/onto/class/google_compute_region_network_endpoint_group"/>
    <rdfs:range rdf:resource="http://www.w3.org/2001/XMLSchema#string"/>
  </owl:DatatypeProperty>
</rdf:RDF>
