<?xml version="1.0" encoding="UTF-8"?>
<rdf:RDF
  xmlns:rdf="http://www.w3.org/1999/02/22-rdf-syntax-ns#"
  xmlns:rdfs="http://www.w3.org/2000/01/rdf-schema#"
  xmlns:owl="http://www.w3.org/2002/07/owl#"
  xmlns:xsd="http://www.w3.org/2001/XMLSchema#"
  xml:base="http://example.org/onto/">
  <owl:Class rdf:about="http://example.org/onto/class/google_network_services_endpoint_policy">
    <rdfs:label>google_network_services_endpoint_policy</rdfs:label>
    <rdfs:comment>#
#     ***     AUTO GENERATED CODE    ***    Type: MMv1     ***
#
# ----------------------------------------------------------------------------
#
#     This code is generated by Magic Modules using the following:
#
#     Configuration: https:#github.com/GoogleCloudPlatform/magic-modules/tree/main/mmv1/products/networkservices/EndpointPolicy.yaml
#     Template:      https:#github.com/GoogleCloudPlatform/magic-modules/tree/main/mmv1/templates/terraform/resource.html.markdown.tmpl
#
#     DO NOT EDIT this file directly. Any changes made to this file will be
#     overwritten during the next generation cycle.
#
# ----------------------------------------------------------------------------
subcategory: "Network Services"
description: |-
  EndpointPolicy is a resource that helps apply desired configuration on the endpoints that match specific criteria.
---</rdfs:comment>
  </owl:Class>
  <owl:DatatypeProperty rdf:about="http://example.org/onto/prop/google_network_services_endpoint_policy_authorization_policy">
    <rdfs:label>authorization_policy</rdfs:label>
    <rdfs:comment>This field specifies the URL of AuthorizationPolicy resource that applies authorization policies to the inbound traffic at the matched endpoints.</rdfs:comment>
    <rdfs:domain rdf:resource="http://example.org/onto/class/google_network_services_endpoint_policy"/>
    <rdfs:range rdf:resource="http://www.w3.org/2001/XMLSchema#string"/>
  </owl:DatatypeProperty>
  <owl:DatatypeProperty rdf:about="http://example.org/onto/prop/google_network_services_endpoint_policy_client_tls_policy">
    <rdfs:label>client_tls_policy</rdfs:label>
    <rdfs:comment>A URL referring to a ClientTlsPolicy resource. ClientTlsPolicy can be set to specify the authentication for traffic from the proxy to the actual endpoints.</rdfs:comment>
    <rdfs:domain rdf:resource="http://example.org/onto/class/google_network_services_endpoint_policy"/>
    <rdfs:range rdf:resource="http://www.w3.org/2001/XMLSchema#string"/>
  </owl:DatatypeProperty>
  <owl:DatatypeProperty rdf:about="http://example.org/onto/prop/google_network_services_endpoint_policy_create_time">
    <rdfs:label>create_time</rdfs:label>
    <rdfs:comment>Time the TcpRoute was created in UTC.</rdfs:comment>
    <rdfs:domain rdf:resource="http://example.org/onto/class/google_network_services_endpoint_policy"/>
    <rdfs:range rdf:resource="http://www.w3.org/2001/XMLSchema#string"/>
  </owl:DatatypeProperty>
  <owl:DatatypeProperty rdf:about="http://example.org/onto/prop/google_network_services_endpoint_policy_description">
    <rdfs:label>description</rdfs:label>
    <rdfs:comment>A free-text description of the resource. Max length 1024 characters.</rdfs:comment>
    <rdfs:domain rdf:resource="http://example.org/onto/class/google_network_services_endpoint_policy"/>
    <rdfs:range rdf:resource="http://www.w3.org/2001/XMLSchema#string"/>
  </owl:DatatypeProperty>
  <owl:DatatypeProperty rdf:about="http://example.org/onto/prop/google_network_services_endpoint_policy_effective_labels">
    <rdfs:label>effective_labels</rdfs:label>
    <rdfs:comment>All of labels (key/value pairs) present on the resource in GCP, including the labels configured through Terraform, other clients and services.</rdfs:comment>
    <rdfs:domain rdf:resource="http://example.org/onto/class/google_network_services_endpoint_policy"/>
    <rdfs:range rdf:resource="http://www.w3.org/2001/XMLSchema#string"/>
  </owl:DatatypeProperty>
  <owl:DatatypeProperty rdf:about="http://example.org/onto/prop/google_network_services_endpoint_policy_id">
    <rdfs:label>id</rdfs:label>
    <rdfs:domain rdf:resource="http://example.org/onto/class/google_network_services_endpoint_policy"/>
    <rdfs:range rdf:resource="http://www.w3.org/2001/XMLSchema#string"/>
  </owl:DatatypeProperty>
  <owl:DatatypeProperty rdf:about="http://example.org/onto/prop/google_network_services_endpoint_policy_labels">
    <rdfs:label>labels</rdfs:label>
    <rdfs:comment>Set of label tags associated with the TcpRoute resource.

**Note**: This field is non-authoritative, and will only manage the labels present in your configuration.
Please refer to the field 'effective_labels' for all of the labels present on the resource.</rdfs:comment>
    <rdfs:domain rdf:resource="http://example.org/onto/class/google_network_services_endpoint_policy"/>
    <rdfs:range rdf:resource="http://www.w3.org/2001/XMLSchema#string"/>
  </owl:DatatypeProperty>
  <owl:DatatypeProperty rdf:about="http://example.org/onto/prop/google_network_services_endpoint_policy_name">
    <rdfs:label>name</rdfs:label>
    <rdfs:comment>Name of the EndpointPolicy resource.</rdfs:comment>
    <rdfs:domain rdf:resource="http://example.org/onto/class/google_network_services_endpoint_policy"/>
    <rdfs:range rdf:resource="http://www.w3.org/2001/XMLSchema#string"/>
  </owl:DatatypeProperty>
  <owl:DatatypeProperty rdf:about="http://example.org/onto/prop/google_network_services_endpoint_policy_project">
    <rdfs:label>project</rdfs:label>
    <rdfs:domain rdf:resource="http://example.org/onto/class/google_network_services_endpoint_policy"/>
    <rdfs:range rdf:resource="http://www.w3.org/2001/XMLSchema#string"/>
  </owl:DatatypeProperty>
  <owl:DatatypeProperty rdf:about="http://example.org/onto/prop/google_network_services_endpoint_policy_server_tls_policy">
    <rdfs:label>server_tls_policy</rdfs:label>
    <rdfs:comment>A URL referring to ServerTlsPolicy resource. ServerTlsPolicy is used to determine the authentication policy to be applied to terminate the inbound traffic at the identified backends.</rdfs:comment>
    <rdfs:domain rdf:resource="http://example.org/onto/class/google_network_services_endpoint_policy"/>
    <rdfs:range rdf:resource="http://www.w3.org/2001/XMLSchema#string"/>
  </owl:DatatypeProperty>
  <owl:DatatypeProperty rdf:about="http://example.org/onto/prop/google_network_services_endpoint_policy_terraform_labels">
    <rdfs:label>terraform_labels</rdfs:label>
    <rdfs:comment>The combination of labels configured directly on the resource
 and default labels configured on the provider.</rdfs:comment>
    <rdfs:domain rdf:resource="http://example.org/onto/class/google_network_services_endpoint_policy"/>
    <rdfs:range rdf:resource="http://www.w3.org/2001/XMLSchema#string"/>
  </owl:DatatypeProperty>
  <owl:DatatypeProperty rdf:about="http://example.org/onto/prop/google_network_services_endpoint_policy_type">
    <rdfs:label>type</rdfs:label>
    <rdfs:comment>The type of endpoint policy. This is primarily used to validate the configuration. Possible values: ["SIDECAR_PROXY", "GRPC_SERVER"]</rdfs:comment>
    <rdfs:domain rdf:resource="http://example.org/onto/class/google_network_services_endpoint_policy"/>
    <rdfs:range rdf:resource="http://www.w3.org/2001/XMLSchema#string"/>
  </owl:DatatypeProperty>
  <owl:DatatypeProperty rdf:about="http://example.org/onto/prop/google_network_services_endpoint_policy_update_time">
    <rdfs:label>update_time</rdfs:label>
    <rdfs:comment>Time the TcpRoute was updated in UTC.</rdfs:comment>
    <rdfs:domain rdf:resource="http://example.org/onto/class/google_network_services_endpoint_policy"/>
    <rdfs:range rdf:resource="http://www.w3.org/2001/XMLSchema#string"/>
  </owl:DatatypeProperty>
  <owl:DatatypeProperty rdf:about="http://example.org/onto/prop/google_network_services_endpoint_policy_metadata_label_match_criteria">
    <rdfs:label>metadata_label_match_criteria</rdfs:label>
    <rdfs:comment>Specifies how matching should be done. Possible values: ["MATCH_ANY", "MATCH_ALL"]</rdfs:comment>
    <rdfs:domain rdf:resource="http://example.org/onto/class/google_network_services_endpoint_policy"/>
    <rdfs:range rdf:resource="http://www.w3.org/2001/XMLSchema#string"/>
  </owl:DatatypeProperty>
  <owl:DatatypeProperty rdf:about="http://example.org/onto/prop/google_network_services_endpoint_policy_label_name">
    <rdfs:label>label_name</rdfs:label>
    <rdfs:comment>Required. Label name presented as key in xDS Node Metadata.</rdfs:comment>
    <rdfs:domain rdf:resource="http://example.org/onto/class/google_network_services_endpoint_policy"/>
    <rdfs:range rdf:resource="http://www.w3.org/2001/XMLSchema#string"/>
  </owl:DatatypeProperty>
  <owl:DatatypeProperty rdf:about="http://example.org/onto/prop/google_network_services_endpoint_policy_label_value">
    <rdfs:label>label_value</rdfs:label>
    <rdfs:comment>Required. Label value presented as value corresponding to the above key, in xDS Node Metadata.</rdfs:comment>
    <rdfs:domain rdf:resource="http://example.org/onto/class/google_network_services_endpoint_policy"/>
    <rdfs:range rdf:resource="http://www.w3.org/2001/XMLSchema#string"/>
  </owl:DatatypeProperty>
  <owl:DatatypeProperty rdf:about="http://example.org/onto/prop/google_network_services_endpoint_policy_create">
    <rdfs:label>create</rdfs:label>
    <rdfs:domain rdf:resource="http://example.org/onto/class/google_network_services_endpoint_policy"/>
    <rdfs:range rdf:resource="http://www.w3.org/2001/XMLSchema#string"/>
  </owl:DatatypeProperty>
  <owl:DatatypeProperty rdf:about="http://example.org/onto/prop/google_network_services_endpoint_policy_delete">
    <rdfs:label>delete</rdfs:label>
    <rdfs:domain rdf:resource="http://example.org/onto/class/google_network_services_endpoint_policy"/>
    <rdfs:range rdf:resource="http://www.w3.org/2001/XMLSchema#string"/>
  </owl:DatatypeProperty>
  <owl:DatatypeProperty rdf:about="http://example.org/onto/prop/google_network_services_endpoint_policy_update">
    <rdfs:label>update</rdfs:label>
    <rdfs:domain rdf:resource="http://example.org/onto/class/google_network_services_endpoint_policy"/>
    <rdfs:range rdf:resource="http://www.w3.org/2001/XMLSchema#string"/>
  </owl:DatatypeProperty>
  <owl:DatatypeProperty rdf:about="http://example.org/onto/prop/google_network_services_endpoint_policy_ports">
    <rdfs:label>ports</rdfs:label>
    <rdfs:comment>List of ports. Can be port numbers or port range (example, [80-90] specifies all ports from 80 to 90, including 80 and 90) or named ports or * to specify all ports. If the list is empty, all ports are selected.</rdfs:comment>
    <rdfs:domain rdf:resource="http://example.org/onto/class/google_network_services_endpoint_policy"/>
    <rdfs:range rdf:resource="http://www.w3.org/2001/XMLSchema#string"/>
  </owl:DatatypeProperty>
</rdf:RDF>
