<?xml version="1.0" encoding="UTF-8"?>
<rdf:RDF
  xmlns:rdf="http://www.w3.org/1999/02/22-rdf-syntax-ns#"
  xmlns:rdfs="http://www.w3.org/2000/01/rdf-schema#"
  xmlns:owl="http://www.w3.org/2002/07/owl#"
  xmlns:xsd="http://www.w3.org/2001/XMLSchema#"
  xml:base="http://example.org/onto/">
  <owl:Class rdf:about="http://example.org/onto/class/google_compute_attached_disk">
    <rdfs:label>google_compute_attached_disk</rdfs:label>
    <rdfs:comment>#
#     ***     AUTO GENERATED CODE    ***    Type: Handwritten     ***
#
# ----------------------------------------------------------------------------
#
#     This code is generated by Magic Modules using the following:
#
#     Source file: https://github.com/GoogleCloudPlatform/magic-modules/tree/main/mmv1/third_party/terraform/website/docs/r/compute_attached_disk.html.markdown
#
#     DO NOT EDIT this file directly. Any changes made to this file will be
#     overwritten during the next generation cycle.
#
# ----------------------------------------------------------------------------
subcategory: "Compute Engine"
description: |-
  Resource that allows attaching existing persistent disks to compute instances.
---</rdfs:comment>
  </owl:Class>
  <owl:DatatypeProperty rdf:about="http://example.org/onto/prop/google_compute_attached_disk_device_name">
    <rdfs:label>device_name</rdfs:label>
    <rdfs:comment>Specifies a unique device name of your choice that is reflected into the /dev/disk/by-id/google-* tree of a Linux operating system running within the instance. This name can be used to reference the device for mounting, resizing, and so on, from within the instance. If not specified, the server chooses a default device name to apply to this disk, in the form persistent-disks-x, where x is a number assigned by Google Compute Engine.</rdfs:comment>
    <rdfs:domain rdf:resource="http://example.org/onto/class/google_compute_attached_disk"/>
    <rdfs:range rdf:resource="http://www.w3.org/2001/XMLSchema#string"/>
  </owl:DatatypeProperty>
  <owl:DatatypeProperty rdf:about="http://example.org/onto/prop/google_compute_attached_disk_disk">
    <rdfs:label>disk</rdfs:label>
    <rdfs:comment>name or self_link of the disk that will be attached.</rdfs:comment>
    <rdfs:domain rdf:resource="http://example.org/onto/class/google_compute_attached_disk"/>
    <rdfs:range rdf:resource="http://www.w3.org/2001/XMLSchema#string"/>
  </owl:DatatypeProperty>
  <owl:DatatypeProperty rdf:about="http://example.org/onto/prop/google_compute_attached_disk_id">
    <rdfs:label>id</rdfs:label>
    <rdfs:domain rdf:resource="http://example.org/onto/class/google_compute_attached_disk"/>
    <rdfs:range rdf:resource="http://www.w3.org/2001/XMLSchema#string"/>
  </owl:DatatypeProperty>
  <owl:DatatypeProperty rdf:about="http://example.org/onto/prop/google_compute_attached_disk_instance">
    <rdfs:label>instance</rdfs:label>
    <rdfs:comment>name or self_link of the compute instance that the disk will be attached to. If the self_link is provided then zone and project are extracted from the self link. If only the name is used then zone and project must be defined as properties on the resource or provider.</rdfs:comment>
    <rdfs:domain rdf:resource="http://example.org/onto/class/google_compute_attached_disk"/>
    <rdfs:range rdf:resource="http://www.w3.org/2001/XMLSchema#string"/>
  </owl:DatatypeProperty>
  <owl:DatatypeProperty rdf:about="http://example.org/onto/prop/google_compute_attached_disk_interface">
    <rdfs:label>interface</rdfs:label>
    <rdfs:comment>The disk interface used for attaching this disk. One of SCSI or NVME. (This field is only used for specific cases, please don't specify this field without advice from Google.)</rdfs:comment>
    <rdfs:domain rdf:resource="http://example.org/onto/class/google_compute_attached_disk"/>
    <rdfs:range rdf:resource="http://www.w3.org/2001/XMLSchema#string"/>
  </owl:DatatypeProperty>
  <owl:DatatypeProperty rdf:about="http://example.org/onto/prop/google_compute_attached_disk_mode">
    <rdfs:label>mode</rdfs:label>
    <rdfs:comment>The mode in which to attach this disk, either READ_WRITE or READ_ONLY. If not specified, the default is to attach the disk in READ_WRITE mode.</rdfs:comment>
    <rdfs:domain rdf:resource="http://example.org/onto/class/google_compute_attached_disk"/>
    <rdfs:range rdf:resource="http://www.w3.org/2001/XMLSchema#string"/>
  </owl:DatatypeProperty>
  <owl:DatatypeProperty rdf:about="http://example.org/onto/prop/google_compute_attached_disk_project">
    <rdfs:label>project</rdfs:label>
    <rdfs:comment>The project that the referenced compute instance is a part of. If instance is referenced by its self_link the project defined in the link will take precedence.</rdfs:comment>
    <rdfs:domain rdf:resource="http://example.org/onto/class/google_compute_attached_disk"/>
    <rdfs:range rdf:resource="http://www.w3.org/2001/XMLSchema#string"/>
  </owl:DatatypeProperty>
  <owl:DatatypeProperty rdf:about="http://example.org/onto/prop/google_compute_attached_disk_zone">
    <rdfs:label>zone</rdfs:label>
    <rdfs:comment>The zone that the referenced compute instance is located within. If instance is referenced by its self_link the zone defined in the link will take precedence.</rdfs:comment>
    <rdfs:domain rdf:resource="http://example.org/onto/class/google_compute_attached_disk"/>
    <rdfs:range rdf:resource="http://www.w3.org/2001/XMLSchema#string"/>
  </owl:DatatypeProperty>
  <owl:DatatypeProperty rdf:about="http://example.org/onto/prop/google_compute_attached_disk_create">
    <rdfs:label>create</rdfs:label>
    <rdfs:domain rdf:resource="http://example.org/onto/class/google_compute_attached_disk"/>
    <rdfs:range rdf:resource="http://www.w3.org/2001/XMLSchema#string"/>
  </owl:DatatypeProperty>
  <owl:DatatypeProperty rdf:about="http://example.org/onto/prop/google_compute_attached_disk_delete">
    <rdfs:label>delete</rdfs:label>
    <rdfs:domain rdf:resource="http://example.org/onto/class/google_compute_attached_disk"/>
    <rdfs:range rdf:resource="http://www.w3.org/2001/XMLSchema#string"/>
  </owl:DatatypeProperty>
</rdf:RDF>
