<?xml version="1.0" encoding="UTF-8"?>
<rdf:RDF
  xmlns:rdf="http://www.w3.org/1999/02/22-rdf-syntax-ns#"
  xmlns:rdfs="http://www.w3.org/2000/01/rdf-schema#"
  xmlns:owl="http://www.w3.org/2002/07/owl#"
  xmlns:xsd="http://www.w3.org/2001/XMLSchema#"
  xml:base="http://example.org/onto/">
  <owl:Class rdf:about="http://example.org/onto/class/google_clouddeploy_target">
    <rdfs:label>google_clouddeploy_target</rdfs:label>
    <rdfs:comment>#
#     ***     AUTO GENERATED CODE    ***    Type: DCL     ***
#
# ----------------------------------------------------------------------------
#
#     This file is managed by Magic Modules (https:#github.com/GoogleCloudPlatform/magic-modules)
#     and is based on the DCL (https:#github.com/GoogleCloudPlatform/declarative-resource-client-library).
#     Changes will need to be made to the DCL or Magic Modules instead of here.
#
#     We are not currently able to accept contributions to this file. If changes
#     are required, please file an issue at https:#github.com/hashicorp/terraform-provider-google/issues/new/choose
#
# ----------------------------------------------------------------------------
subcategory: "Cloud Deploy"
description: |-
  The Cloud Deploy `Target` resource
---</rdfs:comment>
  </owl:Class>
  <owl:DatatypeProperty rdf:about="http://example.org/onto/prop/google_clouddeploy_target_annotations">
    <rdfs:label>annotations</rdfs:label>
    <rdfs:comment>Optional. User annotations. These attributes can only be set and used by the user, and not by Google Cloud Deploy. See https://google.aip.dev/128#annotations for more details such as format and size limitations.

**Note**: This field is non-authoritative, and will only manage the annotations present in your configuration.
Please refer to the field `effective_annotations` for all of the annotations present on the resource.</rdfs:comment>
    <rdfs:domain rdf:resource="http://example.org/onto/class/google_clouddeploy_target"/>
    <rdfs:range rdf:resource="http://www.w3.org/2001/XMLSchema#string"/>
  </owl:DatatypeProperty>
  <owl:DatatypeProperty rdf:about="http://example.org/onto/prop/google_clouddeploy_target_create_time">
    <rdfs:label>create_time</rdfs:label>
    <rdfs:comment>Output only. Time at which the `Target` was created.</rdfs:comment>
    <rdfs:domain rdf:resource="http://example.org/onto/class/google_clouddeploy_target"/>
    <rdfs:range rdf:resource="http://www.w3.org/2001/XMLSchema#string"/>
  </owl:DatatypeProperty>
  <owl:DatatypeProperty rdf:about="http://example.org/onto/prop/google_clouddeploy_target_deploy_parameters">
    <rdfs:label>deploy_parameters</rdfs:label>
    <rdfs:comment>Optional. The deploy parameters to use for this target.</rdfs:comment>
    <rdfs:domain rdf:resource="http://example.org/onto/class/google_clouddeploy_target"/>
    <rdfs:range rdf:resource="http://www.w3.org/2001/XMLSchema#string"/>
  </owl:DatatypeProperty>
  <owl:DatatypeProperty rdf:about="http://example.org/onto/prop/google_clouddeploy_target_description">
    <rdfs:label>description</rdfs:label>
    <rdfs:comment>Optional. Description of the `Target`. Max length is 255 characters.</rdfs:comment>
    <rdfs:domain rdf:resource="http://example.org/onto/class/google_clouddeploy_target"/>
    <rdfs:range rdf:resource="http://www.w3.org/2001/XMLSchema#string"/>
  </owl:DatatypeProperty>
  <owl:DatatypeProperty rdf:about="http://example.org/onto/prop/google_clouddeploy_target_effective_annotations">
    <rdfs:label>effective_annotations</rdfs:label>
    <rdfs:comment>All of annotations (key/value pairs) present on the resource in GCP, including the annotations configured through Terraform, other clients and services.</rdfs:comment>
    <rdfs:domain rdf:resource="http://example.org/onto/class/google_clouddeploy_target"/>
    <rdfs:range rdf:resource="http://www.w3.org/2001/XMLSchema#string"/>
  </owl:DatatypeProperty>
  <owl:DatatypeProperty rdf:about="http://example.org/onto/prop/google_clouddeploy_target_effective_labels">
    <rdfs:label>effective_labels</rdfs:label>
    <rdfs:comment>All of labels (key/value pairs) present on the resource in GCP, including the labels configured through Terraform, other clients and services.</rdfs:comment>
    <rdfs:domain rdf:resource="http://example.org/onto/class/google_clouddeploy_target"/>
    <rdfs:range rdf:resource="http://www.w3.org/2001/XMLSchema#string"/>
  </owl:DatatypeProperty>
  <owl:DatatypeProperty rdf:about="http://example.org/onto/prop/google_clouddeploy_target_etag">
    <rdfs:label>etag</rdfs:label>
    <rdfs:comment>Optional. This checksum is computed by the server based on the value of other fields, and may be sent on update and delete requests to ensure the client has an up-to-date value before proceeding.</rdfs:comment>
    <rdfs:domain rdf:resource="http://example.org/onto/class/google_clouddeploy_target"/>
    <rdfs:range rdf:resource="http://www.w3.org/2001/XMLSchema#string"/>
  </owl:DatatypeProperty>
  <owl:DatatypeProperty rdf:about="http://example.org/onto/prop/google_clouddeploy_target_id">
    <rdfs:label>id</rdfs:label>
    <rdfs:domain rdf:resource="http://example.org/onto/class/google_clouddeploy_target"/>
    <rdfs:range rdf:resource="http://www.w3.org/2001/XMLSchema#string"/>
  </owl:DatatypeProperty>
  <owl:DatatypeProperty rdf:about="http://example.org/onto/prop/google_clouddeploy_target_labels">
    <rdfs:label>labels</rdfs:label>
    <rdfs:comment>Optional. Labels are attributes that can be set and used by both the user and by Google Cloud Deploy. Labels must meet the following constraints: * Keys and values can contain only lowercase letters, numeric characters, underscores, and dashes. * All characters must use UTF-8 encoding, and international characters are allowed. * Keys must start with a lowercase letter or international character. * Each resource is limited to a maximum of 64 labels. Both keys and values are additionally constrained to be <= 128 bytes.

**Note**: This field is non-authoritative, and will only manage the labels present in your configuration.
Please refer to the field `effective_labels` for all of the labels present on the resource.</rdfs:comment>
    <rdfs:domain rdf:resource="http://example.org/onto/class/google_clouddeploy_target"/>
    <rdfs:range rdf:resource="http://www.w3.org/2001/XMLSchema#string"/>
  </owl:DatatypeProperty>
  <owl:DatatypeProperty rdf:about="http://example.org/onto/prop/google_clouddeploy_target_location">
    <rdfs:label>location</rdfs:label>
    <rdfs:comment>The location for the resource</rdfs:comment>
    <rdfs:domain rdf:resource="http://example.org/onto/class/google_clouddeploy_target"/>
    <rdfs:range rdf:resource="http://www.w3.org/2001/XMLSchema#string"/>
  </owl:DatatypeProperty>
  <owl:DatatypeProperty rdf:about="http://example.org/onto/prop/google_clouddeploy_target_name">
    <rdfs:label>name</rdfs:label>
    <rdfs:comment>Name of the `Target`. Format is `[a-z]([a-z0-9-]{0,61}[a-z0-9])?`.</rdfs:comment>
    <rdfs:domain rdf:resource="http://example.org/onto/class/google_clouddeploy_target"/>
    <rdfs:range rdf:resource="http://www.w3.org/2001/XMLSchema#string"/>
  </owl:DatatypeProperty>
  <owl:DatatypeProperty rdf:about="http://example.org/onto/prop/google_clouddeploy_target_project">
    <rdfs:label>project</rdfs:label>
    <rdfs:comment>The project for the resource</rdfs:comment>
    <rdfs:domain rdf:resource="http://example.org/onto/class/google_clouddeploy_target"/>
    <rdfs:range rdf:resource="http://www.w3.org/2001/XMLSchema#string"/>
  </owl:DatatypeProperty>
  <owl:DatatypeProperty rdf:about="http://example.org/onto/prop/google_clouddeploy_target_require_approval">
    <rdfs:label>require_approval</rdfs:label>
    <rdfs:comment>Optional. Whether or not the `Target` requires approval.</rdfs:comment>
    <rdfs:domain rdf:resource="http://example.org/onto/class/google_clouddeploy_target"/>
    <rdfs:range rdf:resource="http://www.w3.org/2001/XMLSchema#string"/>
  </owl:DatatypeProperty>
  <owl:DatatypeProperty rdf:about="http://example.org/onto/prop/google_clouddeploy_target_target_id">
    <rdfs:label>target_id</rdfs:label>
    <rdfs:comment>Output only. Resource id of the `Target`.</rdfs:comment>
    <rdfs:domain rdf:resource="http://example.org/onto/class/google_clouddeploy_target"/>
    <rdfs:range rdf:resource="http://www.w3.org/2001/XMLSchema#string"/>
  </owl:DatatypeProperty>
  <owl:DatatypeProperty rdf:about="http://example.org/onto/prop/google_clouddeploy_target_terraform_labels">
    <rdfs:label>terraform_labels</rdfs:label>
    <rdfs:comment>The combination of labels configured directly on the resource and default labels configured on the provider.</rdfs:comment>
    <rdfs:domain rdf:resource="http://example.org/onto/class/google_clouddeploy_target"/>
    <rdfs:range rdf:resource="http://www.w3.org/2001/XMLSchema#string"/>
  </owl:DatatypeProperty>
  <owl:DatatypeProperty rdf:about="http://example.org/onto/prop/google_clouddeploy_target_uid">
    <rdfs:label>uid</rdfs:label>
    <rdfs:comment>Output only. Unique identifier of the `Target`.</rdfs:comment>
    <rdfs:domain rdf:resource="http://example.org/onto/class/google_clouddeploy_target"/>
    <rdfs:range rdf:resource="http://www.w3.org/2001/XMLSchema#string"/>
  </owl:DatatypeProperty>
  <owl:DatatypeProperty rdf:about="http://example.org/onto/prop/google_clouddeploy_target_update_time">
    <rdfs:label>update_time</rdfs:label>
    <rdfs:comment>Output only. Most recent time at which the `Target` was updated.</rdfs:comment>
    <rdfs:domain rdf:resource="http://example.org/onto/class/google_clouddeploy_target"/>
    <rdfs:range rdf:resource="http://www.w3.org/2001/XMLSchema#string"/>
  </owl:DatatypeProperty>
  <owl:DatatypeProperty rdf:about="http://example.org/onto/prop/google_clouddeploy_target_membership">
    <rdfs:label>membership</rdfs:label>
    <rdfs:comment>Membership of the GKE Hub-registered cluster to which to apply the Skaffold configuration. Format is `projects/{project}/locations/{location}/memberships/{membership_name}`.</rdfs:comment>
    <rdfs:domain rdf:resource="http://example.org/onto/class/google_clouddeploy_target"/>
    <rdfs:range rdf:resource="http://www.w3.org/2001/XMLSchema#string"/>
  </owl:DatatypeProperty>
  <owl:DatatypeProperty rdf:about="http://example.org/onto/prop/google_clouddeploy_target_entity_id">
    <rdfs:label>entity_id</rdfs:label>
    <rdfs:comment>The name for the key in the map for which this object is mapped to in the API</rdfs:comment>
    <rdfs:domain rdf:resource="http://example.org/onto/class/google_clouddeploy_target"/>
    <rdfs:range rdf:resource="http://www.w3.org/2001/XMLSchema#string"/>
  </owl:DatatypeProperty>
  <owl:DatatypeProperty rdf:about="http://example.org/onto/prop/google_clouddeploy_target_membership">
    <rdfs:label>membership</rdfs:label>
    <rdfs:comment>Optional. Membership of the GKE Hub-registered cluster to which to apply the Skaffold configuration. Format is `projects/{project}/locations/{location}/memberships/{membership_name}`.</rdfs:comment>
    <rdfs:domain rdf:resource="http://example.org/onto/class/google_clouddeploy_target"/>
    <rdfs:range rdf:resource="http://www.w3.org/2001/XMLSchema#string"/>
  </owl:DatatypeProperty>
  <owl:DatatypeProperty rdf:about="http://example.org/onto/prop/google_clouddeploy_target_cluster">
    <rdfs:label>cluster</rdfs:label>
    <rdfs:comment>Optional. Information specifying a GKE Cluster. Format is `projects/{project_id}/locations/{location_id}/clusters/{cluster_id}`.</rdfs:comment>
    <rdfs:domain rdf:resource="http://example.org/onto/class/google_clouddeploy_target"/>
    <rdfs:range rdf:resource="http://www.w3.org/2001/XMLSchema#string"/>
  </owl:DatatypeProperty>
  <owl:DatatypeProperty rdf:about="http://example.org/onto/prop/google_clouddeploy_target_internal_ip">
    <rdfs:label>internal_ip</rdfs:label>
    <rdfs:comment>Optional. If true, `cluster` is accessed using the private IP address of the control plane endpoint. Otherwise, the default IP address of the control plane endpoint is used. The default IP address is the private IP address for clusters with private control-plane endpoints and the public IP address otherwise. Only specify this option when `cluster` is a [private GKE cluster](https://cloud.google.com/kubernetes-engine/docs/concepts/private-cluster-concept).</rdfs:comment>
    <rdfs:domain rdf:resource="http://example.org/onto/class/google_clouddeploy_target"/>
    <rdfs:range rdf:resource="http://www.w3.org/2001/XMLSchema#string"/>
  </owl:DatatypeProperty>
  <owl:DatatypeProperty rdf:about="http://example.org/onto/prop/google_clouddeploy_target_proxy_url">
    <rdfs:label>proxy_url</rdfs:label>
    <rdfs:comment>Optional. If set, used to configure a [proxy](https://kubernetes.io/docs/concepts/configuration/organize-cluster-access-kubeconfig/#proxy) to the Kubernetes server.</rdfs:comment>
    <rdfs:domain rdf:resource="http://example.org/onto/class/google_clouddeploy_target"/>
    <rdfs:range rdf:resource="http://www.w3.org/2001/XMLSchema#string"/>
  </owl:DatatypeProperty>
  <owl:DatatypeProperty rdf:about="http://example.org/onto/prop/google_clouddeploy_target_custom_target_type">
    <rdfs:label>custom_target_type</rdfs:label>
    <rdfs:comment>Required. The name of the CustomTargetType. Format must be `projects/{project}/locations/{location}/customTargetTypes/{custom_target_type}`.</rdfs:comment>
    <rdfs:domain rdf:resource="http://example.org/onto/class/google_clouddeploy_target"/>
    <rdfs:range rdf:resource="http://www.w3.org/2001/XMLSchema#string"/>
  </owl:DatatypeProperty>
  <owl:DatatypeProperty rdf:about="http://example.org/onto/prop/google_clouddeploy_target_artifact_storage">
    <rdfs:label>artifact_storage</rdfs:label>
    <rdfs:comment>Optional. Cloud Storage location in which to store execution outputs. This can either be a bucket ("gs://my-bucket") or a path within a bucket ("gs://my-bucket/my-dir"). If unspecified, a default bucket located in the same region will be used.</rdfs:comment>
    <rdfs:domain rdf:resource="http://example.org/onto/class/google_clouddeploy_target"/>
    <rdfs:range rdf:resource="http://www.w3.org/2001/XMLSchema#string"/>
  </owl:DatatypeProperty>
  <owl:DatatypeProperty rdf:about="http://example.org/onto/prop/google_clouddeploy_target_execution_timeout">
    <rdfs:label>execution_timeout</rdfs:label>
    <rdfs:comment>Optional. Execution timeout for a Cloud Build Execution. This must be between 10m and 24h in seconds format. If unspecified, a default timeout of 1h is used.</rdfs:comment>
    <rdfs:domain rdf:resource="http://example.org/onto/class/google_clouddeploy_target"/>
    <rdfs:range rdf:resource="http://www.w3.org/2001/XMLSchema#string"/>
  </owl:DatatypeProperty>
  <owl:DatatypeProperty rdf:about="http://example.org/onto/prop/google_clouddeploy_target_service_account">
    <rdfs:label>service_account</rdfs:label>
    <rdfs:comment>Optional. Google service account to use for execution. If unspecified, the project execution service account (-compute@developer.gserviceaccount.com) is used.</rdfs:comment>
    <rdfs:domain rdf:resource="http://example.org/onto/class/google_clouddeploy_target"/>
    <rdfs:range rdf:resource="http://www.w3.org/2001/XMLSchema#string"/>
  </owl:DatatypeProperty>
  <owl:DatatypeProperty rdf:about="http://example.org/onto/prop/google_clouddeploy_target_usages">
    <rdfs:label>usages</rdfs:label>
    <rdfs:comment>Required. Usages when this configuration should be applied.</rdfs:comment>
    <rdfs:domain rdf:resource="http://example.org/onto/class/google_clouddeploy_target"/>
    <rdfs:range rdf:resource="http://www.w3.org/2001/XMLSchema#string"/>
  </owl:DatatypeProperty>
  <owl:DatatypeProperty rdf:about="http://example.org/onto/prop/google_clouddeploy_target_verbose">
    <rdfs:label>verbose</rdfs:label>
    <rdfs:comment>Optional. If true, additional logging will be enabled when running builds in this execution environment.</rdfs:comment>
    <rdfs:domain rdf:resource="http://example.org/onto/class/google_clouddeploy_target"/>
    <rdfs:range rdf:resource="http://www.w3.org/2001/XMLSchema#string"/>
  </owl:DatatypeProperty>
  <owl:DatatypeProperty rdf:about="http://example.org/onto/prop/google_clouddeploy_target_worker_pool">
    <rdfs:label>worker_pool</rdfs:label>
    <rdfs:comment>Optional. The resource name of the `WorkerPool`, with the format `projects/{project}/locations/{location}/workerPools/{worker_pool}`. If this optional field is unspecified, the default Cloud Build pool will be used.</rdfs:comment>
    <rdfs:domain rdf:resource="http://example.org/onto/class/google_clouddeploy_target"/>
    <rdfs:range rdf:resource="http://www.w3.org/2001/XMLSchema#string"/>
  </owl:DatatypeProperty>
  <owl:DatatypeProperty rdf:about="http://example.org/onto/prop/google_clouddeploy_target_cluster">
    <rdfs:label>cluster</rdfs:label>
    <rdfs:comment>Information specifying a GKE Cluster. Format is `projects/{project_id}/locations/{location_id}/clusters/{cluster_id}.</rdfs:comment>
    <rdfs:domain rdf:resource="http://example.org/onto/class/google_clouddeploy_target"/>
    <rdfs:range rdf:resource="http://www.w3.org/2001/XMLSchema#string"/>
  </owl:DatatypeProperty>
  <owl:DatatypeProperty rdf:about="http://example.org/onto/prop/google_clouddeploy_target_dns_endpoint">
    <rdfs:label>dns_endpoint</rdfs:label>
    <rdfs:comment>Optional. If set, the cluster will be accessed using the DNS endpoint. Note that both `dns_endpoint` and `internal_ip` cannot be set to true.</rdfs:comment>
    <rdfs:domain rdf:resource="http://example.org/onto/class/google_clouddeploy_target"/>
    <rdfs:range rdf:resource="http://www.w3.org/2001/XMLSchema#string"/>
  </owl:DatatypeProperty>
  <owl:DatatypeProperty rdf:about="http://example.org/onto/prop/google_clouddeploy_target_internal_ip">
    <rdfs:label>internal_ip</rdfs:label>
    <rdfs:comment>Optional. If true, `cluster` is accessed using the private IP address of the control plane endpoint. Otherwise, the default IP address of the control plane endpoint is used. The default IP address is the private IP address for clusters with private control-plane endpoints and the public IP address otherwise. Only specify this option when `cluster` is a [private GKE cluster](https://cloud.google.com/kubernetes-engine/docs/concepts/private-cluster-concept).</rdfs:comment>
    <rdfs:domain rdf:resource="http://example.org/onto/class/google_clouddeploy_target"/>
    <rdfs:range rdf:resource="http://www.w3.org/2001/XMLSchema#string"/>
  </owl:DatatypeProperty>
  <owl:DatatypeProperty rdf:about="http://example.org/onto/prop/google_clouddeploy_target_proxy_url">
    <rdfs:label>proxy_url</rdfs:label>
    <rdfs:comment>Optional. If set, used to configure a [proxy](https://kubernetes.io/docs/concepts/configuration/organize-cluster-access-kubeconfig/#proxy) to the Kubernetes server.</rdfs:comment>
    <rdfs:domain rdf:resource="http://example.org/onto/class/google_clouddeploy_target"/>
    <rdfs:range rdf:resource="http://www.w3.org/2001/XMLSchema#string"/>
  </owl:DatatypeProperty>
  <owl:DatatypeProperty rdf:about="http://example.org/onto/prop/google_clouddeploy_target_target_ids">
    <rdfs:label>target_ids</rdfs:label>
    <rdfs:comment>Required. The target_ids of this multiTarget.</rdfs:comment>
    <rdfs:domain rdf:resource="http://example.org/onto/class/google_clouddeploy_target"/>
    <rdfs:range rdf:resource="http://www.w3.org/2001/XMLSchema#string"/>
  </owl:DatatypeProperty>
  <owl:DatatypeProperty rdf:about="http://example.org/onto/prop/google_clouddeploy_target_location">
    <rdfs:label>location</rdfs:label>
    <rdfs:comment>Required. The location where the Cloud Run Service should be located. Format is `projects/{project}/locations/{location}`.</rdfs:comment>
    <rdfs:domain rdf:resource="http://example.org/onto/class/google_clouddeploy_target"/>
    <rdfs:range rdf:resource="http://www.w3.org/2001/XMLSchema#string"/>
  </owl:DatatypeProperty>
  <owl:DatatypeProperty rdf:about="http://example.org/onto/prop/google_clouddeploy_target_create">
    <rdfs:label>create</rdfs:label>
    <rdfs:domain rdf:resource="http://example.org/onto/class/google_clouddeploy_target"/>
    <rdfs:range rdf:resource="http://www.w3.org/2001/XMLSchema#string"/>
  </owl:DatatypeProperty>
  <owl:DatatypeProperty rdf:about="http://example.org/onto/prop/google_clouddeploy_target_delete">
    <rdfs:label>delete</rdfs:label>
    <rdfs:domain rdf:resource="http://example.org/onto/class/google_clouddeploy_target"/>
    <rdfs:range rdf:resource="http://www.w3.org/2001/XMLSchema#string"/>
  </owl:DatatypeProperty>
  <owl:DatatypeProperty rdf:about="http://example.org/onto/prop/google_clouddeploy_target_update">
    <rdfs:label>update</rdfs:label>
    <rdfs:domain rdf:resource="http://example.org/onto/class/google_clouddeploy_target"/>
    <rdfs:range rdf:resource="http://www.w3.org/2001/XMLSchema#string"/>
  </owl:DatatypeProperty>
</rdf:RDF>
