<?xml version="1.0" encoding="UTF-8"?>
<rdf:RDF
  xmlns:rdf="http://www.w3.org/1999/02/22-rdf-syntax-ns#"
  xmlns:rdfs="http://www.w3.org/2000/01/rdf-schema#"
  xmlns:owl="http://www.w3.org/2002/07/owl#"
  xmlns:xsd="http://www.w3.org/2001/XMLSchema#"
  xml:base="http://example.org/onto/">
  <owl:Class rdf:about="http://example.org/onto/class/google_iam_principal_access_boundary_policy">
    <rdfs:label>google_iam_principal_access_boundary_policy</rdfs:label>
    <rdfs:comment>#
#     ***     AUTO GENERATED CODE    ***    Type: MMv1     ***
#
# ----------------------------------------------------------------------------
#
#     This code is generated by Magic Modules using the following:
#
#     Configuration: https:#github.com/GoogleCloudPlatform/magic-modules/tree/main/mmv1/products/iam3/PrincipalAccessBoundaryPolicy.yaml
#     Template:      https:#github.com/GoogleCloudPlatform/magic-modules/tree/main/mmv1/templates/terraform/resource.html.markdown.tmpl
#
#     DO NOT EDIT this file directly. Any changes made to this file will be
#     overwritten during the next generation cycle.
#
# ----------------------------------------------------------------------------
subcategory: "Cloud IAM"
description: |-
  An IAM Principal Access Boundary Policy resource.
---</rdfs:comment>
  </owl:Class>
  <owl:DatatypeProperty rdf:about="http://example.org/onto/prop/google_iam_principal_access_boundary_policy_annotations">
    <rdfs:label>annotations</rdfs:label>
    <rdfs:comment>User defined annotations. See https://google.aip.dev/148#annotations
for more details such as format and size limitations


**Note**: This field is non-authoritative, and will only manage the annotations present in your configuration.
Please refer to the field 'effective_annotations' for all of the annotations present on the resource.</rdfs:comment>
    <rdfs:domain rdf:resource="http://example.org/onto/class/google_iam_principal_access_boundary_policy"/>
    <rdfs:range rdf:resource="http://www.w3.org/2001/XMLSchema#string"/>
  </owl:DatatypeProperty>
  <owl:DatatypeProperty rdf:about="http://example.org/onto/prop/google_iam_principal_access_boundary_policy_create_time">
    <rdfs:label>create_time</rdfs:label>
    <rdfs:comment>Output only. The time when the principal access boundary policy was created.</rdfs:comment>
    <rdfs:domain rdf:resource="http://example.org/onto/class/google_iam_principal_access_boundary_policy"/>
    <rdfs:range rdf:resource="http://www.w3.org/2001/XMLSchema#string"/>
  </owl:DatatypeProperty>
  <owl:DatatypeProperty rdf:about="http://example.org/onto/prop/google_iam_principal_access_boundary_policy_display_name">
    <rdfs:label>display_name</rdfs:label>
    <rdfs:comment>The description of the principal access boundary policy. Must be less than or equal to 63 characters.</rdfs:comment>
    <rdfs:domain rdf:resource="http://example.org/onto/class/google_iam_principal_access_boundary_policy"/>
    <rdfs:range rdf:resource="http://www.w3.org/2001/XMLSchema#string"/>
  </owl:DatatypeProperty>
  <owl:DatatypeProperty rdf:about="http://example.org/onto/prop/google_iam_principal_access_boundary_policy_effective_annotations">
    <rdfs:label>effective_annotations</rdfs:label>
    <rdfs:comment>All of annotations (key/value pairs) present on the resource in GCP, including the annotations configured through Terraform, other clients and services.</rdfs:comment>
    <rdfs:domain rdf:resource="http://example.org/onto/class/google_iam_principal_access_boundary_policy"/>
    <rdfs:range rdf:resource="http://www.w3.org/2001/XMLSchema#string"/>
  </owl:DatatypeProperty>
  <owl:DatatypeProperty rdf:about="http://example.org/onto/prop/google_iam_principal_access_boundary_policy_etag">
    <rdfs:label>etag</rdfs:label>
    <rdfs:comment>The etag for the principal access boundary. If this is provided on update, it must match the server's etag.</rdfs:comment>
    <rdfs:domain rdf:resource="http://example.org/onto/class/google_iam_principal_access_boundary_policy"/>
    <rdfs:range rdf:resource="http://www.w3.org/2001/XMLSchema#string"/>
  </owl:DatatypeProperty>
  <owl:DatatypeProperty rdf:about="http://example.org/onto/prop/google_iam_principal_access_boundary_policy_id">
    <rdfs:label>id</rdfs:label>
    <rdfs:domain rdf:resource="http://example.org/onto/class/google_iam_principal_access_boundary_policy"/>
    <rdfs:range rdf:resource="http://www.w3.org/2001/XMLSchema#string"/>
  </owl:DatatypeProperty>
  <owl:DatatypeProperty rdf:about="http://example.org/onto/prop/google_iam_principal_access_boundary_policy_location">
    <rdfs:label>location</rdfs:label>
    <rdfs:comment>The location the principal access boundary policy is in.</rdfs:comment>
    <rdfs:domain rdf:resource="http://example.org/onto/class/google_iam_principal_access_boundary_policy"/>
    <rdfs:range rdf:resource="http://www.w3.org/2001/XMLSchema#string"/>
  </owl:DatatypeProperty>
  <owl:DatatypeProperty rdf:about="http://example.org/onto/prop/google_iam_principal_access_boundary_policy_name">
    <rdfs:label>name</rdfs:label>
    <rdfs:comment>Identifier. The resource name of the principal access boundary policy.  The following format is supported:
 'organizations/{organization_id}/locations/{location}/principalAccessBoundaryPolicies/{policy_id}'</rdfs:comment>
    <rdfs:domain rdf:resource="http://example.org/onto/class/google_iam_principal_access_boundary_policy"/>
    <rdfs:range rdf:resource="http://www.w3.org/2001/XMLSchema#string"/>
  </owl:DatatypeProperty>
  <owl:DatatypeProperty rdf:about="http://example.org/onto/prop/google_iam_principal_access_boundary_policy_organization">
    <rdfs:label>organization</rdfs:label>
    <rdfs:comment>The parent organization of the principal access boundary policy.</rdfs:comment>
    <rdfs:domain rdf:resource="http://example.org/onto/class/google_iam_principal_access_boundary_policy"/>
    <rdfs:range rdf:resource="http://www.w3.org/2001/XMLSchema#string"/>
  </owl:DatatypeProperty>
  <owl:DatatypeProperty rdf:about="http://example.org/onto/prop/google_iam_principal_access_boundary_policy_principal_access_boundary_policy_id">
    <rdfs:label>principal_access_boundary_policy_id</rdfs:label>
    <rdfs:comment>The ID to use to create the principal access boundary policy.
This value must start with a lowercase letter followed by up to 62 lowercase letters, numbers, hyphens, or dots. Pattern, /a-z{2,62}/.</rdfs:comment>
    <rdfs:domain rdf:resource="http://example.org/onto/class/google_iam_principal_access_boundary_policy"/>
    <rdfs:range rdf:resource="http://www.w3.org/2001/XMLSchema#string"/>
  </owl:DatatypeProperty>
  <owl:DatatypeProperty rdf:about="http://example.org/onto/prop/google_iam_principal_access_boundary_policy_uid">
    <rdfs:label>uid</rdfs:label>
    <rdfs:comment>Output only. The globally unique ID of the principal access boundary policy.</rdfs:comment>
    <rdfs:domain rdf:resource="http://example.org/onto/class/google_iam_principal_access_boundary_policy"/>
    <rdfs:range rdf:resource="http://www.w3.org/2001/XMLSchema#string"/>
  </owl:DatatypeProperty>
  <owl:DatatypeProperty rdf:about="http://example.org/onto/prop/google_iam_principal_access_boundary_policy_update_time">
    <rdfs:label>update_time</rdfs:label>
    <rdfs:comment>Output only. The time when the principal access boundary policy was most recently updated.</rdfs:comment>
    <rdfs:domain rdf:resource="http://example.org/onto/class/google_iam_principal_access_boundary_policy"/>
    <rdfs:range rdf:resource="http://www.w3.org/2001/XMLSchema#string"/>
  </owl:DatatypeProperty>
  <owl:DatatypeProperty rdf:about="http://example.org/onto/prop/google_iam_principal_access_boundary_policy_enforcement_version">
    <rdfs:label>enforcement_version</rdfs:label>
    <rdfs:comment>The version number that indicates which Google Cloud services
are included in the enforcement (e.g. \"latest\", \"1\", ...). If empty, the
PAB policy version will be set to the current latest version, and this version
won't get updated when new versions are released.</rdfs:comment>
    <rdfs:domain rdf:resource="http://example.org/onto/class/google_iam_principal_access_boundary_policy"/>
    <rdfs:range rdf:resource="http://www.w3.org/2001/XMLSchema#string"/>
  </owl:DatatypeProperty>
  <owl:DatatypeProperty rdf:about="http://example.org/onto/prop/google_iam_principal_access_boundary_policy_description">
    <rdfs:label>description</rdfs:label>
    <rdfs:comment>The description of the principal access boundary policy rule. Must be less than or equal to 256 characters.</rdfs:comment>
    <rdfs:domain rdf:resource="http://example.org/onto/class/google_iam_principal_access_boundary_policy"/>
    <rdfs:range rdf:resource="http://www.w3.org/2001/XMLSchema#string"/>
  </owl:DatatypeProperty>
  <owl:DatatypeProperty rdf:about="http://example.org/onto/prop/google_iam_principal_access_boundary_policy_effect">
    <rdfs:label>effect</rdfs:label>
    <rdfs:comment>The access relationship of principals to the resources in this rule.
Possible values: ALLOW</rdfs:comment>
    <rdfs:domain rdf:resource="http://example.org/onto/class/google_iam_principal_access_boundary_policy"/>
    <rdfs:range rdf:resource="http://www.w3.org/2001/XMLSchema#string"/>
  </owl:DatatypeProperty>
  <owl:DatatypeProperty rdf:about="http://example.org/onto/prop/google_iam_principal_access_boundary_policy_resources">
    <rdfs:label>resources</rdfs:label>
    <rdfs:comment>A list of Cloud Resource Manager resources. The resource
and all the descendants are included. The number of resources in a policy
is limited to 500 across all rules.
The following resource types are supported:
* Organizations, such as '//cloudresourcemanager.googleapis.com/organizations/123'.
* Folders, such as '//cloudresourcemanager.googleapis.com/folders/123'.
* Projects, such as '//cloudresourcemanager.googleapis.com/projects/123'
or '//cloudresourcemanager.googleapis.com/projects/my-project-id'.</rdfs:comment>
    <rdfs:domain rdf:resource="http://example.org/onto/class/google_iam_principal_access_boundary_policy"/>
    <rdfs:range rdf:resource="http://www.w3.org/2001/XMLSchema#string"/>
  </owl:DatatypeProperty>
  <owl:DatatypeProperty rdf:about="http://example.org/onto/prop/google_iam_principal_access_boundary_policy_create">
    <rdfs:label>create</rdfs:label>
    <rdfs:domain rdf:resource="http://example.org/onto/class/google_iam_principal_access_boundary_policy"/>
    <rdfs:range rdf:resource="http://www.w3.org/2001/XMLSchema#string"/>
  </owl:DatatypeProperty>
  <owl:DatatypeProperty rdf:about="http://example.org/onto/prop/google_iam_principal_access_boundary_policy_delete">
    <rdfs:label>delete</rdfs:label>
    <rdfs:domain rdf:resource="http://example.org/onto/class/google_iam_principal_access_boundary_policy"/>
    <rdfs:range rdf:resource="http://www.w3.org/2001/XMLSchema#string"/>
  </owl:DatatypeProperty>
  <owl:DatatypeProperty rdf:about="http://example.org/onto/prop/google_iam_principal_access_boundary_policy_update">
    <rdfs:label>update</rdfs:label>
    <rdfs:domain rdf:resource="http://example.org/onto/class/google_iam_principal_access_boundary_policy"/>
    <rdfs:range rdf:resource="http://www.w3.org/2001/XMLSchema#string"/>
  </owl:DatatypeProperty>
</rdf:RDF>
