<?xml version="1.0" encoding="UTF-8"?>
<rdf:RDF
  xmlns:rdf="http://www.w3.org/1999/02/22-rdf-syntax-ns#"
  xmlns:rdfs="http://www.w3.org/2000/01/rdf-schema#"
  xmlns:owl="http://www.w3.org/2002/07/owl#"
  xmlns:xsd="http://www.w3.org/2001/XMLSchema#"
  xml:base="http://example.org/onto/">
  <owl:Class rdf:about="http://example.org/onto/class/google_discovery_engine_chat_engine">
    <rdfs:label>google_discovery_engine_chat_engine</rdfs:label>
    <rdfs:comment>#
#     ***     AUTO GENERATED CODE    ***    Type: MMv1     ***
#
# ----------------------------------------------------------------------------
#
#     This code is generated by Magic Modules using the following:
#
#     Configuration: https:#github.com/GoogleCloudPlatform/magic-modules/tree/main/mmv1/products/discoveryengine/ChatEngine.yaml
#     Template:      https:#github.com/GoogleCloudPlatform/magic-modules/tree/main/mmv1/templates/terraform/resource.html.markdown.tmpl
#
#     DO NOT EDIT this file directly. Any changes made to this file will be
#     overwritten during the next generation cycle.
#
# ----------------------------------------------------------------------------
subcategory: "Discovery Engine"
description: |-
  Vertex chat and Conversation Engine Chat type
---</rdfs:comment>
  </owl:Class>
  <owl:DatatypeProperty rdf:about="http://example.org/onto/prop/google_discovery_engine_chat_engine_chat_engine_metadata">
    <rdfs:label>chat_engine_metadata</rdfs:label>
    <rdfs:comment>Additional information of the Chat Engine.</rdfs:comment>
    <rdfs:domain rdf:resource="http://example.org/onto/class/google_discovery_engine_chat_engine"/>
    <rdfs:range rdf:resource="http://www.w3.org/2001/XMLSchema#string"/>
  </owl:DatatypeProperty>
  <owl:DatatypeProperty rdf:about="http://example.org/onto/prop/google_discovery_engine_chat_engine_collection_id">
    <rdfs:label>collection_id</rdfs:label>
    <rdfs:comment>The collection ID.</rdfs:comment>
    <rdfs:domain rdf:resource="http://example.org/onto/class/google_discovery_engine_chat_engine"/>
    <rdfs:range rdf:resource="http://www.w3.org/2001/XMLSchema#string"/>
  </owl:DatatypeProperty>
  <owl:DatatypeProperty rdf:about="http://example.org/onto/prop/google_discovery_engine_chat_engine_create_time">
    <rdfs:label>create_time</rdfs:label>
    <rdfs:comment>Timestamp the Engine was created at.</rdfs:comment>
    <rdfs:domain rdf:resource="http://example.org/onto/class/google_discovery_engine_chat_engine"/>
    <rdfs:range rdf:resource="http://www.w3.org/2001/XMLSchema#string"/>
  </owl:DatatypeProperty>
  <owl:DatatypeProperty rdf:about="http://example.org/onto/prop/google_discovery_engine_chat_engine_data_store_ids">
    <rdfs:label>data_store_ids</rdfs:label>
    <rdfs:comment>The data stores associated with this engine. Multiple DataStores in the same Collection can be associated here. All listed DataStores must be 'SOLUTION_TYPE_CHAT'.</rdfs:comment>
    <rdfs:domain rdf:resource="http://example.org/onto/class/google_discovery_engine_chat_engine"/>
    <rdfs:range rdf:resource="http://www.w3.org/2001/XMLSchema#string"/>
  </owl:DatatypeProperty>
  <owl:DatatypeProperty rdf:about="http://example.org/onto/prop/google_discovery_engine_chat_engine_display_name">
    <rdfs:label>display_name</rdfs:label>
    <rdfs:comment>The display name of the engine. Should be human readable. UTF-8 encoded string with limit of 1024 characters.</rdfs:comment>
    <rdfs:domain rdf:resource="http://example.org/onto/class/google_discovery_engine_chat_engine"/>
    <rdfs:range rdf:resource="http://www.w3.org/2001/XMLSchema#string"/>
  </owl:DatatypeProperty>
  <owl:DatatypeProperty rdf:about="http://example.org/onto/prop/google_discovery_engine_chat_engine_engine_id">
    <rdfs:label>engine_id</rdfs:label>
    <rdfs:comment>The ID to use for chat engine.</rdfs:comment>
    <rdfs:domain rdf:resource="http://example.org/onto/class/google_discovery_engine_chat_engine"/>
    <rdfs:range rdf:resource="http://www.w3.org/2001/XMLSchema#string"/>
  </owl:DatatypeProperty>
  <owl:DatatypeProperty rdf:about="http://example.org/onto/prop/google_discovery_engine_chat_engine_id">
    <rdfs:label>id</rdfs:label>
    <rdfs:domain rdf:resource="http://example.org/onto/class/google_discovery_engine_chat_engine"/>
    <rdfs:range rdf:resource="http://www.w3.org/2001/XMLSchema#string"/>
  </owl:DatatypeProperty>
  <owl:DatatypeProperty rdf:about="http://example.org/onto/prop/google_discovery_engine_chat_engine_industry_vertical">
    <rdfs:label>industry_vertical</rdfs:label>
    <rdfs:comment>The industry vertical that the chat engine registers. Vertical on Engine has to match vertical of the DataStore linked to the engine. Default value: "GENERIC" Possible values: ["GENERIC"]</rdfs:comment>
    <rdfs:domain rdf:resource="http://example.org/onto/class/google_discovery_engine_chat_engine"/>
    <rdfs:range rdf:resource="http://www.w3.org/2001/XMLSchema#string"/>
  </owl:DatatypeProperty>
  <owl:DatatypeProperty rdf:about="http://example.org/onto/prop/google_discovery_engine_chat_engine_location">
    <rdfs:label>location</rdfs:label>
    <rdfs:comment>Location.</rdfs:comment>
    <rdfs:domain rdf:resource="http://example.org/onto/class/google_discovery_engine_chat_engine"/>
    <rdfs:range rdf:resource="http://www.w3.org/2001/XMLSchema#string"/>
  </owl:DatatypeProperty>
  <owl:DatatypeProperty rdf:about="http://example.org/onto/prop/google_discovery_engine_chat_engine_name">
    <rdfs:label>name</rdfs:label>
    <rdfs:comment>The unique full resource name of the chat engine. Values are of the format
'projects/{project}/locations/{location}/collections/{collection_id}/engines/{engine_id}'.
This field must be a UTF-8 encoded string with a length limit of 1024
characters.</rdfs:comment>
    <rdfs:domain rdf:resource="http://example.org/onto/class/google_discovery_engine_chat_engine"/>
    <rdfs:range rdf:resource="http://www.w3.org/2001/XMLSchema#string"/>
  </owl:DatatypeProperty>
  <owl:DatatypeProperty rdf:about="http://example.org/onto/prop/google_discovery_engine_chat_engine_project">
    <rdfs:label>project</rdfs:label>
    <rdfs:domain rdf:resource="http://example.org/onto/class/google_discovery_engine_chat_engine"/>
    <rdfs:range rdf:resource="http://www.w3.org/2001/XMLSchema#string"/>
  </owl:DatatypeProperty>
  <owl:DatatypeProperty rdf:about="http://example.org/onto/prop/google_discovery_engine_chat_engine_update_time">
    <rdfs:label>update_time</rdfs:label>
    <rdfs:comment>Timestamp the Engine was last updated.</rdfs:comment>
    <rdfs:domain rdf:resource="http://example.org/onto/class/google_discovery_engine_chat_engine"/>
    <rdfs:range rdf:resource="http://www.w3.org/2001/XMLSchema#string"/>
  </owl:DatatypeProperty>
  <owl:DatatypeProperty rdf:about="http://example.org/onto/prop/google_discovery_engine_chat_engine_allow_cross_region">
    <rdfs:label>allow_cross_region</rdfs:label>
    <rdfs:comment>If the flag set to true, we allow the agent and engine are in
different locations, otherwise the agent and engine are required to be
in the same location. The flag is set to false by default.
Note that the 'allow_cross_region' are one-time consumed by and passed
to EngineService.CreateEngine. It means they cannot be retrieved using
EngineService.GetEngine or EngineService.ListEngines API after engine
creation.</rdfs:comment>
    <rdfs:domain rdf:resource="http://example.org/onto/class/google_discovery_engine_chat_engine"/>
    <rdfs:range rdf:resource="http://www.w3.org/2001/XMLSchema#string"/>
  </owl:DatatypeProperty>
  <owl:DatatypeProperty rdf:about="http://example.org/onto/prop/google_discovery_engine_chat_engine_dialogflow_agent_to_link">
    <rdfs:label>dialogflow_agent_to_link</rdfs:label>
    <rdfs:comment>The resource name of an existing Dialogflow agent to link to this Chat Engine. Format: 'projects/<Project_ID>/locations/<Location_ID>/agents/<Agent_ID>'.
Exactly one of 'agent_creation_config' or 'dialogflow_agent_to_link' must be set.</rdfs:comment>
    <rdfs:domain rdf:resource="http://example.org/onto/class/google_discovery_engine_chat_engine"/>
    <rdfs:range rdf:resource="http://www.w3.org/2001/XMLSchema#string"/>
  </owl:DatatypeProperty>
  <owl:DatatypeProperty rdf:about="http://example.org/onto/prop/google_discovery_engine_chat_engine_business">
    <rdfs:label>business</rdfs:label>
    <rdfs:comment>Name of the company, organization or other entity that the agent represents. Used for knowledge connector LLM prompt and for knowledge search.</rdfs:comment>
    <rdfs:domain rdf:resource="http://example.org/onto/class/google_discovery_engine_chat_engine"/>
    <rdfs:range rdf:resource="http://www.w3.org/2001/XMLSchema#string"/>
  </owl:DatatypeProperty>
  <owl:DatatypeProperty rdf:about="http://example.org/onto/prop/google_discovery_engine_chat_engine_default_language_code">
    <rdfs:label>default_language_code</rdfs:label>
    <rdfs:comment>The default language of the agent as a language tag. See [Language Support](https://cloud.google.com/dialogflow/docs/reference/language) for a list of the currently supported language codes.</rdfs:comment>
    <rdfs:domain rdf:resource="http://example.org/onto/class/google_discovery_engine_chat_engine"/>
    <rdfs:range rdf:resource="http://www.w3.org/2001/XMLSchema#string"/>
  </owl:DatatypeProperty>
  <owl:DatatypeProperty rdf:about="http://example.org/onto/prop/google_discovery_engine_chat_engine_location">
    <rdfs:label>location</rdfs:label>
    <rdfs:comment>Agent location for Agent creation, currently supported values: global/us/eu, it needs to be the same region as the Chat Engine.</rdfs:comment>
    <rdfs:domain rdf:resource="http://example.org/onto/class/google_discovery_engine_chat_engine"/>
    <rdfs:range rdf:resource="http://www.w3.org/2001/XMLSchema#string"/>
  </owl:DatatypeProperty>
  <owl:DatatypeProperty rdf:about="http://example.org/onto/prop/google_discovery_engine_chat_engine_time_zone">
    <rdfs:label>time_zone</rdfs:label>
    <rdfs:comment>The time zone of the agent from the [time zone database](https://www.iana.org/time-zones), e.g., America/New_York, Europe/Paris.</rdfs:comment>
    <rdfs:domain rdf:resource="http://example.org/onto/class/google_discovery_engine_chat_engine"/>
    <rdfs:range rdf:resource="http://www.w3.org/2001/XMLSchema#string"/>
  </owl:DatatypeProperty>
  <owl:DatatypeProperty rdf:about="http://example.org/onto/prop/google_discovery_engine_chat_engine_company_name">
    <rdfs:label>company_name</rdfs:label>
    <rdfs:comment>The name of the company, business or entity that is associated with the engine. Setting this may help improve LLM related features.</rdfs:comment>
    <rdfs:domain rdf:resource="http://example.org/onto/class/google_discovery_engine_chat_engine"/>
    <rdfs:range rdf:resource="http://www.w3.org/2001/XMLSchema#string"/>
  </owl:DatatypeProperty>
  <owl:DatatypeProperty rdf:about="http://example.org/onto/prop/google_discovery_engine_chat_engine_create">
    <rdfs:label>create</rdfs:label>
    <rdfs:domain rdf:resource="http://example.org/onto/class/google_discovery_engine_chat_engine"/>
    <rdfs:range rdf:resource="http://www.w3.org/2001/XMLSchema#string"/>
  </owl:DatatypeProperty>
  <owl:DatatypeProperty rdf:about="http://example.org/onto/prop/google_discovery_engine_chat_engine_delete">
    <rdfs:label>delete</rdfs:label>
    <rdfs:domain rdf:resource="http://example.org/onto/class/google_discovery_engine_chat_engine"/>
    <rdfs:range rdf:resource="http://www.w3.org/2001/XMLSchema#string"/>
  </owl:DatatypeProperty>
  <owl:DatatypeProperty rdf:about="http://example.org/onto/prop/google_discovery_engine_chat_engine_update">
    <rdfs:label>update</rdfs:label>
    <rdfs:domain rdf:resource="http://example.org/onto/class/google_discovery_engine_chat_engine"/>
    <rdfs:range rdf:resource="http://www.w3.org/2001/XMLSchema#string"/>
  </owl:DatatypeProperty>
</rdf:RDF>
