<?xml version="1.0" encoding="UTF-8"?>
<rdf:RDF
  xmlns:rdf="http://www.w3.org/1999/02/22-rdf-syntax-ns#"
  xmlns:rdfs="http://www.w3.org/2000/01/rdf-schema#"
  xmlns:owl="http://www.w3.org/2002/07/owl#"
  xmlns:xsd="http://www.w3.org/2001/XMLSchema#"
  xml:base="http://example.org/onto/">
  <owl:Class rdf:about="http://example.org/onto/class/google_securityposture_posture">
    <rdfs:label>google_securityposture_posture</rdfs:label>
    <rdfs:comment>#
#     ***     AUTO GENERATED CODE    ***    Type: MMv1     ***
#
# ----------------------------------------------------------------------------
#
#     This code is generated by Magic Modules using the following:
#
#     Configuration: https:#github.com/GoogleCloudPlatform/magic-modules/tree/main/mmv1/products/securityposture/Posture.yaml
#     Template:      https:#github.com/GoogleCloudPlatform/magic-modules/tree/main/mmv1/templates/terraform/resource.html.markdown.tmpl
#
#     DO NOT EDIT this file directly. Any changes made to this file will be
#     overwritten during the next generation cycle.
#
# ----------------------------------------------------------------------------
subcategory: "Security Posture"
description: |-
  A Posture represents a collection of policy set including its name, state, description
  and policy sets.
---</rdfs:comment>
  </owl:Class>
  <owl:DatatypeProperty rdf:about="http://example.org/onto/prop/google_securityposture_posture_create_time">
    <rdfs:label>create_time</rdfs:label>
    <rdfs:comment>Time the Posture was created in UTC.</rdfs:comment>
    <rdfs:domain rdf:resource="http://example.org/onto/class/google_securityposture_posture"/>
    <rdfs:range rdf:resource="http://www.w3.org/2001/XMLSchema#string"/>
  </owl:DatatypeProperty>
  <owl:DatatypeProperty rdf:about="http://example.org/onto/prop/google_securityposture_posture_description">
    <rdfs:label>description</rdfs:label>
    <rdfs:comment>Description of the posture.</rdfs:comment>
    <rdfs:domain rdf:resource="http://example.org/onto/class/google_securityposture_posture"/>
    <rdfs:range rdf:resource="http://www.w3.org/2001/XMLSchema#string"/>
  </owl:DatatypeProperty>
  <owl:DatatypeProperty rdf:about="http://example.org/onto/prop/google_securityposture_posture_etag">
    <rdfs:label>etag</rdfs:label>
    <rdfs:comment>For Resource freshness validation (https://google.aip.dev/154)</rdfs:comment>
    <rdfs:domain rdf:resource="http://example.org/onto/class/google_securityposture_posture"/>
    <rdfs:range rdf:resource="http://www.w3.org/2001/XMLSchema#string"/>
  </owl:DatatypeProperty>
  <owl:DatatypeProperty rdf:about="http://example.org/onto/prop/google_securityposture_posture_id">
    <rdfs:label>id</rdfs:label>
    <rdfs:domain rdf:resource="http://example.org/onto/class/google_securityposture_posture"/>
    <rdfs:range rdf:resource="http://www.w3.org/2001/XMLSchema#string"/>
  </owl:DatatypeProperty>
  <owl:DatatypeProperty rdf:about="http://example.org/onto/prop/google_securityposture_posture_location">
    <rdfs:label>location</rdfs:label>
    <rdfs:comment>Location of the resource, eg: global.</rdfs:comment>
    <rdfs:domain rdf:resource="http://example.org/onto/class/google_securityposture_posture"/>
    <rdfs:range rdf:resource="http://www.w3.org/2001/XMLSchema#string"/>
  </owl:DatatypeProperty>
  <owl:DatatypeProperty rdf:about="http://example.org/onto/prop/google_securityposture_posture_name">
    <rdfs:label>name</rdfs:label>
    <rdfs:comment>Name of the posture.</rdfs:comment>
    <rdfs:domain rdf:resource="http://example.org/onto/class/google_securityposture_posture"/>
    <rdfs:range rdf:resource="http://www.w3.org/2001/XMLSchema#string"/>
  </owl:DatatypeProperty>
  <owl:DatatypeProperty rdf:about="http://example.org/onto/prop/google_securityposture_posture_parent">
    <rdfs:label>parent</rdfs:label>
    <rdfs:comment>The parent of the resource, an organization. Format should be 'organizations/{organization_id}'.</rdfs:comment>
    <rdfs:domain rdf:resource="http://example.org/onto/class/google_securityposture_posture"/>
    <rdfs:range rdf:resource="http://www.w3.org/2001/XMLSchema#string"/>
  </owl:DatatypeProperty>
  <owl:DatatypeProperty rdf:about="http://example.org/onto/prop/google_securityposture_posture_posture_id">
    <rdfs:label>posture_id</rdfs:label>
    <rdfs:comment>Id of the posture. It is an immutable field.</rdfs:comment>
    <rdfs:domain rdf:resource="http://example.org/onto/class/google_securityposture_posture"/>
    <rdfs:range rdf:resource="http://www.w3.org/2001/XMLSchema#string"/>
  </owl:DatatypeProperty>
  <owl:DatatypeProperty rdf:about="http://example.org/onto/prop/google_securityposture_posture_reconciling">
    <rdfs:label>reconciling</rdfs:label>
    <rdfs:comment>If set, there are currently changes in flight to the posture.</rdfs:comment>
    <rdfs:domain rdf:resource="http://example.org/onto/class/google_securityposture_posture"/>
    <rdfs:range rdf:resource="http://www.w3.org/2001/XMLSchema#string"/>
  </owl:DatatypeProperty>
  <owl:DatatypeProperty rdf:about="http://example.org/onto/prop/google_securityposture_posture_revision_id">
    <rdfs:label>revision_id</rdfs:label>
    <rdfs:comment>Revision_id of the posture.</rdfs:comment>
    <rdfs:domain rdf:resource="http://example.org/onto/class/google_securityposture_posture"/>
    <rdfs:range rdf:resource="http://www.w3.org/2001/XMLSchema#string"/>
  </owl:DatatypeProperty>
  <owl:DatatypeProperty rdf:about="http://example.org/onto/prop/google_securityposture_posture_state">
    <rdfs:label>state</rdfs:label>
    <rdfs:comment>State of the posture. Update to state field should not be triggered along with
with other field updates. Possible values: ["DEPRECATED", "DRAFT", "ACTIVE"]</rdfs:comment>
    <rdfs:domain rdf:resource="http://example.org/onto/class/google_securityposture_posture"/>
    <rdfs:range rdf:resource="http://www.w3.org/2001/XMLSchema#string"/>
  </owl:DatatypeProperty>
  <owl:DatatypeProperty rdf:about="http://example.org/onto/prop/google_securityposture_posture_update_time">
    <rdfs:label>update_time</rdfs:label>
    <rdfs:comment>Time the Posture was updated in UTC.</rdfs:comment>
    <rdfs:domain rdf:resource="http://example.org/onto/class/google_securityposture_posture"/>
    <rdfs:range rdf:resource="http://www.w3.org/2001/XMLSchema#string"/>
  </owl:DatatypeProperty>
  <owl:DatatypeProperty rdf:about="http://example.org/onto/prop/google_securityposture_posture_description">
    <rdfs:label>description</rdfs:label>
    <rdfs:comment>Description of the policy set.</rdfs:comment>
    <rdfs:domain rdf:resource="http://example.org/onto/class/google_securityposture_posture"/>
    <rdfs:range rdf:resource="http://www.w3.org/2001/XMLSchema#string"/>
  </owl:DatatypeProperty>
  <owl:DatatypeProperty rdf:about="http://example.org/onto/prop/google_securityposture_posture_policy_set_id">
    <rdfs:label>policy_set_id</rdfs:label>
    <rdfs:comment>ID of the policy set.</rdfs:comment>
    <rdfs:domain rdf:resource="http://example.org/onto/class/google_securityposture_posture"/>
    <rdfs:range rdf:resource="http://www.w3.org/2001/XMLSchema#string"/>
  </owl:DatatypeProperty>
  <owl:DatatypeProperty rdf:about="http://example.org/onto/prop/google_securityposture_posture_description">
    <rdfs:label>description</rdfs:label>
    <rdfs:comment>Description of the policy.</rdfs:comment>
    <rdfs:domain rdf:resource="http://example.org/onto/class/google_securityposture_posture"/>
    <rdfs:range rdf:resource="http://www.w3.org/2001/XMLSchema#string"/>
  </owl:DatatypeProperty>
  <owl:DatatypeProperty rdf:about="http://example.org/onto/prop/google_securityposture_posture_policy_id">
    <rdfs:label>policy_id</rdfs:label>
    <rdfs:comment>ID of the policy.</rdfs:comment>
    <rdfs:domain rdf:resource="http://example.org/onto/class/google_securityposture_posture"/>
    <rdfs:range rdf:resource="http://www.w3.org/2001/XMLSchema#string"/>
  </owl:DatatypeProperty>
  <owl:DatatypeProperty rdf:about="http://example.org/onto/prop/google_securityposture_posture_control">
    <rdfs:label>control</rdfs:label>
    <rdfs:comment>Mapping of security controls for the policy.</rdfs:comment>
    <rdfs:domain rdf:resource="http://example.org/onto/class/google_securityposture_posture"/>
    <rdfs:range rdf:resource="http://www.w3.org/2001/XMLSchema#string"/>
  </owl:DatatypeProperty>
  <owl:DatatypeProperty rdf:about="http://example.org/onto/prop/google_securityposture_posture_standard">
    <rdfs:label>standard</rdfs:label>
    <rdfs:comment>Mapping of compliance standards for the policy.</rdfs:comment>
    <rdfs:domain rdf:resource="http://example.org/onto/class/google_securityposture_posture"/>
    <rdfs:range rdf:resource="http://www.w3.org/2001/XMLSchema#string"/>
  </owl:DatatypeProperty>
  <owl:DatatypeProperty rdf:about="http://example.org/onto/prop/google_securityposture_posture_canned_constraint_id">
    <rdfs:label>canned_constraint_id</rdfs:label>
    <rdfs:comment>Organization policy canned constraint Id</rdfs:comment>
    <rdfs:domain rdf:resource="http://example.org/onto/class/google_securityposture_posture"/>
    <rdfs:range rdf:resource="http://www.w3.org/2001/XMLSchema#string"/>
  </owl:DatatypeProperty>
  <owl:DatatypeProperty rdf:about="http://example.org/onto/prop/google_securityposture_posture_allow_all">
    <rdfs:label>allow_all</rdfs:label>
    <rdfs:comment>Setting this to true means that all values are allowed. This field can be set only in policies for list constraints.</rdfs:comment>
    <rdfs:domain rdf:resource="http://example.org/onto/class/google_securityposture_posture"/>
    <rdfs:range rdf:resource="http://www.w3.org/2001/XMLSchema#string"/>
  </owl:DatatypeProperty>
  <owl:DatatypeProperty rdf:about="http://example.org/onto/prop/google_securityposture_posture_deny_all">
    <rdfs:label>deny_all</rdfs:label>
    <rdfs:comment>Setting this to true means that all values are denied. This field can be set only in policies for list constraints.</rdfs:comment>
    <rdfs:domain rdf:resource="http://example.org/onto/class/google_securityposture_posture"/>
    <rdfs:range rdf:resource="http://www.w3.org/2001/XMLSchema#string"/>
  </owl:DatatypeProperty>
  <owl:DatatypeProperty rdf:about="http://example.org/onto/prop/google_securityposture_posture_enforce">
    <rdfs:label>enforce</rdfs:label>
    <rdfs:comment>If 'true', then the policy is enforced. If 'false', then any configuration is acceptable.
This field can be set only in policies for boolean constraints.</rdfs:comment>
    <rdfs:domain rdf:resource="http://example.org/onto/class/google_securityposture_posture"/>
    <rdfs:range rdf:resource="http://www.w3.org/2001/XMLSchema#string"/>
  </owl:DatatypeProperty>
  <owl:DatatypeProperty rdf:about="http://example.org/onto/prop/google_securityposture_posture_description">
    <rdfs:label>description</rdfs:label>
    <rdfs:comment>Description of the expression</rdfs:comment>
    <rdfs:domain rdf:resource="http://example.org/onto/class/google_securityposture_posture"/>
    <rdfs:range rdf:resource="http://www.w3.org/2001/XMLSchema#string"/>
  </owl:DatatypeProperty>
  <owl:DatatypeProperty rdf:about="http://example.org/onto/prop/google_securityposture_posture_expression">
    <rdfs:label>expression</rdfs:label>
    <rdfs:comment>Textual representation of an expression in Common Expression Language syntax.</rdfs:comment>
    <rdfs:domain rdf:resource="http://example.org/onto/class/google_securityposture_posture"/>
    <rdfs:range rdf:resource="http://www.w3.org/2001/XMLSchema#string"/>
  </owl:DatatypeProperty>
  <owl:DatatypeProperty rdf:about="http://example.org/onto/prop/google_securityposture_posture_location">
    <rdfs:label>location</rdfs:label>
    <rdfs:comment>String indicating the location of the expression for error reporting, e.g. a file name and a position in the file</rdfs:comment>
    <rdfs:domain rdf:resource="http://example.org/onto/class/google_securityposture_posture"/>
    <rdfs:range rdf:resource="http://www.w3.org/2001/XMLSchema#string"/>
  </owl:DatatypeProperty>
  <owl:DatatypeProperty rdf:about="http://example.org/onto/prop/google_securityposture_posture_title">
    <rdfs:label>title</rdfs:label>
    <rdfs:comment>Title for the expression, i.e. a short string describing its purpose.</rdfs:comment>
    <rdfs:domain rdf:resource="http://example.org/onto/class/google_securityposture_posture"/>
    <rdfs:range rdf:resource="http://www.w3.org/2001/XMLSchema#string"/>
  </owl:DatatypeProperty>
  <owl:DatatypeProperty rdf:about="http://example.org/onto/prop/google_securityposture_posture_allowed_values">
    <rdfs:label>allowed_values</rdfs:label>
    <rdfs:comment>List of values allowed at this resource.</rdfs:comment>
    <rdfs:domain rdf:resource="http://example.org/onto/class/google_securityposture_posture"/>
    <rdfs:range rdf:resource="http://www.w3.org/2001/XMLSchema#string"/>
  </owl:DatatypeProperty>
  <owl:DatatypeProperty rdf:about="http://example.org/onto/prop/google_securityposture_posture_denied_values">
    <rdfs:label>denied_values</rdfs:label>
    <rdfs:comment>List of values denied at this resource.</rdfs:comment>
    <rdfs:domain rdf:resource="http://example.org/onto/class/google_securityposture_posture"/>
    <rdfs:range rdf:resource="http://www.w3.org/2001/XMLSchema#string"/>
  </owl:DatatypeProperty>
  <owl:DatatypeProperty rdf:about="http://example.org/onto/prop/google_securityposture_posture_action_type">
    <rdfs:label>action_type</rdfs:label>
    <rdfs:comment>The action to take if the condition is met. Possible values: ["ALLOW", "DENY"]</rdfs:comment>
    <rdfs:domain rdf:resource="http://example.org/onto/class/google_securityposture_posture"/>
    <rdfs:range rdf:resource="http://www.w3.org/2001/XMLSchema#string"/>
  </owl:DatatypeProperty>
  <owl:DatatypeProperty rdf:about="http://example.org/onto/prop/google_securityposture_posture_condition">
    <rdfs:label>condition</rdfs:label>
    <rdfs:comment>A CEL condition that refers to a supported service resource, for example 'resource.management.autoUpgrade == false'. For details about CEL usage, see [Common Expression Language](https://cloud.google.com/resource-manager/docs/organization-policy/creating-managing-custom-constraints#common_expression_language).</rdfs:comment>
    <rdfs:domain rdf:resource="http://example.org/onto/class/google_securityposture_posture"/>
    <rdfs:range rdf:resource="http://www.w3.org/2001/XMLSchema#string"/>
  </owl:DatatypeProperty>
  <owl:DatatypeProperty rdf:about="http://example.org/onto/prop/google_securityposture_posture_description">
    <rdfs:label>description</rdfs:label>
    <rdfs:comment>A human-friendly description of the constraint to display as an error message when the policy is violated.</rdfs:comment>
    <rdfs:domain rdf:resource="http://example.org/onto/class/google_securityposture_posture"/>
    <rdfs:range rdf:resource="http://www.w3.org/2001/XMLSchema#string"/>
  </owl:DatatypeProperty>
  <owl:DatatypeProperty rdf:about="http://example.org/onto/prop/google_securityposture_posture_display_name">
    <rdfs:label>display_name</rdfs:label>
    <rdfs:comment>A human-friendly name for the constraint.</rdfs:comment>
    <rdfs:domain rdf:resource="http://example.org/onto/class/google_securityposture_posture"/>
    <rdfs:range rdf:resource="http://www.w3.org/2001/XMLSchema#string"/>
  </owl:DatatypeProperty>
  <owl:DatatypeProperty rdf:about="http://example.org/onto/prop/google_securityposture_posture_method_types">
    <rdfs:label>method_types</rdfs:label>
    <rdfs:comment>A list of RESTful methods for which to enforce the constraint. Can be 'CREATE', 'UPDATE', or both. Not all Google Cloud services support both methods. To see supported methods for each service, find the service in [Supported services](https://cloud.google.com/resource-manager/docs/organization-policy/custom-constraint-supported-services).</rdfs:comment>
    <rdfs:domain rdf:resource="http://example.org/onto/class/google_securityposture_posture"/>
    <rdfs:range rdf:resource="http://www.w3.org/2001/XMLSchema#string"/>
  </owl:DatatypeProperty>
  <owl:DatatypeProperty rdf:about="http://example.org/onto/prop/google_securityposture_posture_name">
    <rdfs:label>name</rdfs:label>
    <rdfs:comment>Immutable. The name of the custom constraint. This is unique within the organization.</rdfs:comment>
    <rdfs:domain rdf:resource="http://example.org/onto/class/google_securityposture_posture"/>
    <rdfs:range rdf:resource="http://www.w3.org/2001/XMLSchema#string"/>
  </owl:DatatypeProperty>
  <owl:DatatypeProperty rdf:about="http://example.org/onto/prop/google_securityposture_posture_resource_types">
    <rdfs:label>resource_types</rdfs:label>
    <rdfs:comment>Immutable. The fully qualified name of the Google Cloud REST resource containing the object and field you want to restrict. For example, 'container.googleapis.com/NodePool'.</rdfs:comment>
    <rdfs:domain rdf:resource="http://example.org/onto/class/google_securityposture_posture"/>
    <rdfs:range rdf:resource="http://www.w3.org/2001/XMLSchema#string"/>
  </owl:DatatypeProperty>
  <owl:DatatypeProperty rdf:about="http://example.org/onto/prop/google_securityposture_posture_allow_all">
    <rdfs:label>allow_all</rdfs:label>
    <rdfs:comment>Setting this to true means that all values are allowed. This field can be set only in policies for list constraints.</rdfs:comment>
    <rdfs:domain rdf:resource="http://example.org/onto/class/google_securityposture_posture"/>
    <rdfs:range rdf:resource="http://www.w3.org/2001/XMLSchema#string"/>
  </owl:DatatypeProperty>
  <owl:DatatypeProperty rdf:about="http://example.org/onto/prop/google_securityposture_posture_deny_all">
    <rdfs:label>deny_all</rdfs:label>
    <rdfs:comment>Setting this to true means that all values are denied. This field can be set only in policies for list constraints.</rdfs:comment>
    <rdfs:domain rdf:resource="http://example.org/onto/class/google_securityposture_posture"/>
    <rdfs:range rdf:resource="http://www.w3.org/2001/XMLSchema#string"/>
  </owl:DatatypeProperty>
  <owl:DatatypeProperty rdf:about="http://example.org/onto/prop/google_securityposture_posture_enforce">
    <rdfs:label>enforce</rdfs:label>
    <rdfs:comment>If 'true', then the policy is enforced. If 'false', then any configuration is acceptable.
This field can be set only in policies for boolean constraints.</rdfs:comment>
    <rdfs:domain rdf:resource="http://example.org/onto/class/google_securityposture_posture"/>
    <rdfs:range rdf:resource="http://www.w3.org/2001/XMLSchema#string"/>
  </owl:DatatypeProperty>
  <owl:DatatypeProperty rdf:about="http://example.org/onto/prop/google_securityposture_posture_description">
    <rdfs:label>description</rdfs:label>
    <rdfs:comment>Description of the expression</rdfs:comment>
    <rdfs:domain rdf:resource="http://example.org/onto/class/google_securityposture_posture"/>
    <rdfs:range rdf:resource="http://www.w3.org/2001/XMLSchema#string"/>
  </owl:DatatypeProperty>
  <owl:DatatypeProperty rdf:about="http://example.org/onto/prop/google_securityposture_posture_expression">
    <rdfs:label>expression</rdfs:label>
    <rdfs:comment>Textual representation of an expression in Common Expression Language syntax.</rdfs:comment>
    <rdfs:domain rdf:resource="http://example.org/onto/class/google_securityposture_posture"/>
    <rdfs:range rdf:resource="http://www.w3.org/2001/XMLSchema#string"/>
  </owl:DatatypeProperty>
  <owl:DatatypeProperty rdf:about="http://example.org/onto/prop/google_securityposture_posture_location">
    <rdfs:label>location</rdfs:label>
    <rdfs:comment>String indicating the location of the expression for error reporting, e.g. a file name and a position in the file</rdfs:comment>
    <rdfs:domain rdf:resource="http://example.org/onto/class/google_securityposture_posture"/>
    <rdfs:range rdf:resource="http://www.w3.org/2001/XMLSchema#string"/>
  </owl:DatatypeProperty>
  <owl:DatatypeProperty rdf:about="http://example.org/onto/prop/google_securityposture_posture_title">
    <rdfs:label>title</rdfs:label>
    <rdfs:comment>Title for the expression, i.e. a short string describing its purpose.</rdfs:comment>
    <rdfs:domain rdf:resource="http://example.org/onto/class/google_securityposture_posture"/>
    <rdfs:range rdf:resource="http://www.w3.org/2001/XMLSchema#string"/>
  </owl:DatatypeProperty>
  <owl:DatatypeProperty rdf:about="http://example.org/onto/prop/google_securityposture_posture_allowed_values">
    <rdfs:label>allowed_values</rdfs:label>
    <rdfs:comment>List of values allowed at this resource.</rdfs:comment>
    <rdfs:domain rdf:resource="http://example.org/onto/class/google_securityposture_posture"/>
    <rdfs:range rdf:resource="http://www.w3.org/2001/XMLSchema#string"/>
  </owl:DatatypeProperty>
  <owl:DatatypeProperty rdf:about="http://example.org/onto/prop/google_securityposture_posture_denied_values">
    <rdfs:label>denied_values</rdfs:label>
    <rdfs:comment>List of values denied at this resource.</rdfs:comment>
    <rdfs:domain rdf:resource="http://example.org/onto/class/google_securityposture_posture"/>
    <rdfs:range rdf:resource="http://www.w3.org/2001/XMLSchema#string"/>
  </owl:DatatypeProperty>
  <owl:DatatypeProperty rdf:about="http://example.org/onto/prop/google_securityposture_posture_display_name">
    <rdfs:label>display_name</rdfs:label>
    <rdfs:comment>The display name of the Security Health Analytics custom module. This
display name becomes the finding category for all findings that are
returned by this custom module.</rdfs:comment>
    <rdfs:domain rdf:resource="http://example.org/onto/class/google_securityposture_posture"/>
    <rdfs:range rdf:resource="http://www.w3.org/2001/XMLSchema#string"/>
  </owl:DatatypeProperty>
  <owl:DatatypeProperty rdf:about="http://example.org/onto/prop/google_securityposture_posture_id">
    <rdfs:label>id</rdfs:label>
    <rdfs:comment>A server generated id of custom module.</rdfs:comment>
    <rdfs:domain rdf:resource="http://example.org/onto/class/google_securityposture_posture"/>
    <rdfs:range rdf:resource="http://www.w3.org/2001/XMLSchema#string"/>
  </owl:DatatypeProperty>
  <owl:DatatypeProperty rdf:about="http://example.org/onto/prop/google_securityposture_posture_module_enablement_state">
    <rdfs:label>module_enablement_state</rdfs:label>
    <rdfs:comment>The state of enablement for the module at its level of the resource hierarchy. Possible values: ["ENABLEMENT_STATE_UNSPECIFIED", "ENABLED", "DISABLED"]</rdfs:comment>
    <rdfs:domain rdf:resource="http://example.org/onto/class/google_securityposture_posture"/>
    <rdfs:range rdf:resource="http://www.w3.org/2001/XMLSchema#string"/>
  </owl:DatatypeProperty>
  <owl:DatatypeProperty rdf:about="http://example.org/onto/prop/google_securityposture_posture_description">
    <rdfs:label>description</rdfs:label>
    <rdfs:comment>Text that describes the vulnerability or misconfiguration that the custom
module detects.</rdfs:comment>
    <rdfs:domain rdf:resource="http://example.org/onto/class/google_securityposture_posture"/>
    <rdfs:range rdf:resource="http://www.w3.org/2001/XMLSchema#string"/>
  </owl:DatatypeProperty>
  <owl:DatatypeProperty rdf:about="http://example.org/onto/prop/google_securityposture_posture_recommendation">
    <rdfs:label>recommendation</rdfs:label>
    <rdfs:comment>An explanation of the recommended steps that security teams can take to
resolve the detected issue</rdfs:comment>
    <rdfs:domain rdf:resource="http://example.org/onto/class/google_securityposture_posture"/>
    <rdfs:range rdf:resource="http://www.w3.org/2001/XMLSchema#string"/>
  </owl:DatatypeProperty>
  <owl:DatatypeProperty rdf:about="http://example.org/onto/prop/google_securityposture_posture_severity">
    <rdfs:label>severity</rdfs:label>
    <rdfs:comment>The severity to assign to findings generated by the module. Possible values: ["SEVERITY_UNSPECIFIED", "CRITICAL", "HIGH", "MEDIUM", "LOW"]</rdfs:comment>
    <rdfs:domain rdf:resource="http://example.org/onto/class/google_securityposture_posture"/>
    <rdfs:range rdf:resource="http://www.w3.org/2001/XMLSchema#string"/>
  </owl:DatatypeProperty>
  <owl:DatatypeProperty rdf:about="http://example.org/onto/prop/google_securityposture_posture_name">
    <rdfs:label>name</rdfs:label>
    <rdfs:comment>Name of the property for the custom output.</rdfs:comment>
    <rdfs:domain rdf:resource="http://example.org/onto/class/google_securityposture_posture"/>
    <rdfs:range rdf:resource="http://www.w3.org/2001/XMLSchema#string"/>
  </owl:DatatypeProperty>
  <owl:DatatypeProperty rdf:about="http://example.org/onto/prop/google_securityposture_posture_description">
    <rdfs:label>description</rdfs:label>
    <rdfs:comment>Description of the expression</rdfs:comment>
    <rdfs:domain rdf:resource="http://example.org/onto/class/google_securityposture_posture"/>
    <rdfs:range rdf:resource="http://www.w3.org/2001/XMLSchema#string"/>
  </owl:DatatypeProperty>
  <owl:DatatypeProperty rdf:about="http://example.org/onto/prop/google_securityposture_posture_expression">
    <rdfs:label>expression</rdfs:label>
    <rdfs:comment>Textual representation of an expression in Common Expression Language syntax.</rdfs:comment>
    <rdfs:domain rdf:resource="http://example.org/onto/class/google_securityposture_posture"/>
    <rdfs:range rdf:resource="http://www.w3.org/2001/XMLSchema#string"/>
  </owl:DatatypeProperty>
  <owl:DatatypeProperty rdf:about="http://example.org/onto/prop/google_securityposture_posture_location">
    <rdfs:label>location</rdfs:label>
    <rdfs:comment>String indicating the location of the expression for error reporting, e.g. a file name and a position in the file</rdfs:comment>
    <rdfs:domain rdf:resource="http://example.org/onto/class/google_securityposture_posture"/>
    <rdfs:range rdf:resource="http://www.w3.org/2001/XMLSchema#string"/>
  </owl:DatatypeProperty>
  <owl:DatatypeProperty rdf:about="http://example.org/onto/prop/google_securityposture_posture_title">
    <rdfs:label>title</rdfs:label>
    <rdfs:comment>Title for the expression, i.e. a short string describing its purpose.</rdfs:comment>
    <rdfs:domain rdf:resource="http://example.org/onto/class/google_securityposture_posture"/>
    <rdfs:range rdf:resource="http://www.w3.org/2001/XMLSchema#string"/>
  </owl:DatatypeProperty>
  <owl:DatatypeProperty rdf:about="http://example.org/onto/prop/google_securityposture_posture_description">
    <rdfs:label>description</rdfs:label>
    <rdfs:comment>Description of the expression</rdfs:comment>
    <rdfs:domain rdf:resource="http://example.org/onto/class/google_securityposture_posture"/>
    <rdfs:range rdf:resource="http://www.w3.org/2001/XMLSchema#string"/>
  </owl:DatatypeProperty>
  <owl:DatatypeProperty rdf:about="http://example.org/onto/prop/google_securityposture_posture_expression">
    <rdfs:label>expression</rdfs:label>
    <rdfs:comment>Textual representation of an expression in Common Expression Language syntax.</rdfs:comment>
    <rdfs:domain rdf:resource="http://example.org/onto/class/google_securityposture_posture"/>
    <rdfs:range rdf:resource="http://www.w3.org/2001/XMLSchema#string"/>
  </owl:DatatypeProperty>
  <owl:DatatypeProperty rdf:about="http://example.org/onto/prop/google_securityposture_posture_location">
    <rdfs:label>location</rdfs:label>
    <rdfs:comment>String indicating the location of the expression for error reporting, e.g. a file name and a position in the file</rdfs:comment>
    <rdfs:domain rdf:resource="http://example.org/onto/class/google_securityposture_posture"/>
    <rdfs:range rdf:resource="http://www.w3.org/2001/XMLSchema#string"/>
  </owl:DatatypeProperty>
  <owl:DatatypeProperty rdf:about="http://example.org/onto/prop/google_securityposture_posture_title">
    <rdfs:label>title</rdfs:label>
    <rdfs:comment>Title for the expression, i.e. a short string describing its purpose.</rdfs:comment>
    <rdfs:domain rdf:resource="http://example.org/onto/class/google_securityposture_posture"/>
    <rdfs:range rdf:resource="http://www.w3.org/2001/XMLSchema#string"/>
  </owl:DatatypeProperty>
  <owl:DatatypeProperty rdf:about="http://example.org/onto/prop/google_securityposture_posture_resource_types">
    <rdfs:label>resource_types</rdfs:label>
    <rdfs:comment>The resource types to run the detector on.</rdfs:comment>
    <rdfs:domain rdf:resource="http://example.org/onto/class/google_securityposture_posture"/>
    <rdfs:range rdf:resource="http://www.w3.org/2001/XMLSchema#string"/>
  </owl:DatatypeProperty>
  <owl:DatatypeProperty rdf:about="http://example.org/onto/prop/google_securityposture_posture_module_enablement_state">
    <rdfs:label>module_enablement_state</rdfs:label>
    <rdfs:comment>The state of enablement for the module at its level of the resource hierarchy. Possible values: ["ENABLEMENT_STATE_UNSPECIFIED", "ENABLED", "DISABLED"]</rdfs:comment>
    <rdfs:domain rdf:resource="http://example.org/onto/class/google_securityposture_posture"/>
    <rdfs:range rdf:resource="http://www.w3.org/2001/XMLSchema#string"/>
  </owl:DatatypeProperty>
  <owl:DatatypeProperty rdf:about="http://example.org/onto/prop/google_securityposture_posture_module_name">
    <rdfs:label>module_name</rdfs:label>
    <rdfs:comment>The name of the module eg: BIGQUERY_TABLE_CMEK_DISABLED.</rdfs:comment>
    <rdfs:domain rdf:resource="http://example.org/onto/class/google_securityposture_posture"/>
    <rdfs:range rdf:resource="http://www.w3.org/2001/XMLSchema#string"/>
  </owl:DatatypeProperty>
  <owl:DatatypeProperty rdf:about="http://example.org/onto/prop/google_securityposture_posture_create">
    <rdfs:label>create</rdfs:label>
    <rdfs:domain rdf:resource="http://example.org/onto/class/google_securityposture_posture"/>
    <rdfs:range rdf:resource="http://www.w3.org/2001/XMLSchema#string"/>
  </owl:DatatypeProperty>
  <owl:DatatypeProperty rdf:about="http://example.org/onto/prop/google_securityposture_posture_delete">
    <rdfs:label>delete</rdfs:label>
    <rdfs:domain rdf:resource="http://example.org/onto/class/google_securityposture_posture"/>
    <rdfs:range rdf:resource="http://www.w3.org/2001/XMLSchema#string"/>
  </owl:DatatypeProperty>
  <owl:DatatypeProperty rdf:about="http://example.org/onto/prop/google_securityposture_posture_update">
    <rdfs:label>update</rdfs:label>
    <rdfs:domain rdf:resource="http://example.org/onto/class/google_securityposture_posture"/>
    <rdfs:range rdf:resource="http://www.w3.org/2001/XMLSchema#string"/>
  </owl:DatatypeProperty>
</rdf:RDF>
