<?xml version="1.0" encoding="UTF-8"?>
<rdf:RDF
  xmlns:rdf="http://www.w3.org/1999/02/22-rdf-syntax-ns#"
  xmlns:rdfs="http://www.w3.org/2000/01/rdf-schema#"
  xmlns:owl="http://www.w3.org/2002/07/owl#"
  xmlns:xsd="http://www.w3.org/2001/XMLSchema#"
  xml:base="http://example.org/onto/">
  <owl:Class rdf:about="http://example.org/onto/class/google_kms_crypto_key_version">
    <rdfs:label>google_kms_crypto_key_version</rdfs:label>
    <rdfs:comment>#
#     ***     AUTO GENERATED CODE    ***    Type: MMv1     ***
#
# ----------------------------------------------------------------------------
#
#     This code is generated by Magic Modules using the following:
#
#     Configuration: https:#github.com/GoogleCloudPlatform/magic-modules/tree/main/mmv1/products/kms/CryptoKeyVersion.yaml
#     Template:      https:#github.com/GoogleCloudPlatform/magic-modules/tree/main/mmv1/templates/terraform/resource.html.markdown.tmpl
#
#     DO NOT EDIT this file directly. Any changes made to this file will be
#     overwritten during the next generation cycle.
#
# ----------------------------------------------------------------------------
subcategory: "Cloud Key Management Service"
description: |-
  A `CryptoKeyVersion` represents an individual cryptographic key, and the associated key material.
---</rdfs:comment>
  </owl:Class>
  <owl:DatatypeProperty rdf:about="http://example.org/onto/prop/google_kms_crypto_key_version_algorithm">
    <rdfs:label>algorithm</rdfs:label>
    <rdfs:comment>The CryptoKeyVersionAlgorithm that this CryptoKeyVersion supports.</rdfs:comment>
    <rdfs:domain rdf:resource="http://example.org/onto/class/google_kms_crypto_key_version"/>
    <rdfs:range rdf:resource="http://www.w3.org/2001/XMLSchema#string"/>
  </owl:DatatypeProperty>
  <owl:DatatypeProperty rdf:about="http://example.org/onto/prop/google_kms_crypto_key_version_attestation">
    <rdfs:label>attestation</rdfs:label>
    <rdfs:comment>Statement that was generated and signed by the HSM at key creation time. Use this statement to verify attributes of the key as stored on the HSM, independently of Google.
Only provided for key versions with protectionLevel HSM.</rdfs:comment>
    <rdfs:domain rdf:resource="http://example.org/onto/class/google_kms_crypto_key_version"/>
    <rdfs:range rdf:resource="http://www.w3.org/2001/XMLSchema#string"/>
  </owl:DatatypeProperty>
  <owl:DatatypeProperty rdf:about="http://example.org/onto/prop/google_kms_crypto_key_version_crypto_key">
    <rdfs:label>crypto_key</rdfs:label>
    <rdfs:comment>The name of the cryptoKey associated with the CryptoKeyVersions.
Format: ''projects/{{project}}/locations/{{location}}/keyRings/{{keyring}}/cryptoKeys/{{cryptoKey}}''</rdfs:comment>
    <rdfs:domain rdf:resource="http://example.org/onto/class/google_kms_crypto_key_version"/>
    <rdfs:range rdf:resource="http://www.w3.org/2001/XMLSchema#string"/>
  </owl:DatatypeProperty>
  <owl:DatatypeProperty rdf:about="http://example.org/onto/prop/google_kms_crypto_key_version_generate_time">
    <rdfs:label>generate_time</rdfs:label>
    <rdfs:comment>The time this CryptoKeyVersion key material was generated</rdfs:comment>
    <rdfs:domain rdf:resource="http://example.org/onto/class/google_kms_crypto_key_version"/>
    <rdfs:range rdf:resource="http://www.w3.org/2001/XMLSchema#string"/>
  </owl:DatatypeProperty>
  <owl:DatatypeProperty rdf:about="http://example.org/onto/prop/google_kms_crypto_key_version_id">
    <rdfs:label>id</rdfs:label>
    <rdfs:domain rdf:resource="http://example.org/onto/class/google_kms_crypto_key_version"/>
    <rdfs:range rdf:resource="http://www.w3.org/2001/XMLSchema#string"/>
  </owl:DatatypeProperty>
  <owl:DatatypeProperty rdf:about="http://example.org/onto/prop/google_kms_crypto_key_version_name">
    <rdfs:label>name</rdfs:label>
    <rdfs:comment>The resource name for this CryptoKeyVersion.</rdfs:comment>
    <rdfs:domain rdf:resource="http://example.org/onto/class/google_kms_crypto_key_version"/>
    <rdfs:range rdf:resource="http://www.w3.org/2001/XMLSchema#string"/>
  </owl:DatatypeProperty>
  <owl:DatatypeProperty rdf:about="http://example.org/onto/prop/google_kms_crypto_key_version_protection_level">
    <rdfs:label>protection_level</rdfs:label>
    <rdfs:comment>The ProtectionLevel describing how crypto operations are performed with this CryptoKeyVersion.</rdfs:comment>
    <rdfs:domain rdf:resource="http://example.org/onto/class/google_kms_crypto_key_version"/>
    <rdfs:range rdf:resource="http://www.w3.org/2001/XMLSchema#string"/>
  </owl:DatatypeProperty>
  <owl:DatatypeProperty rdf:about="http://example.org/onto/prop/google_kms_crypto_key_version_state">
    <rdfs:label>state</rdfs:label>
    <rdfs:comment>The current state of the CryptoKeyVersion. Note: you can only specify this field to manually 'ENABLE' or 'DISABLE' the CryptoKeyVersion,
otherwise the value of this field is always retrieved automatically. Possible values: ["PENDING_GENERATION", "ENABLED", "DISABLED", "DESTROYED", "DESTROY_SCHEDULED", "PENDING_IMPORT", "IMPORT_FAILED"]</rdfs:comment>
    <rdfs:domain rdf:resource="http://example.org/onto/class/google_kms_crypto_key_version"/>
    <rdfs:range rdf:resource="http://www.w3.org/2001/XMLSchema#string"/>
  </owl:DatatypeProperty>
  <owl:DatatypeProperty rdf:about="http://example.org/onto/prop/google_kms_crypto_key_version_ekm_connection_key_path">
    <rdfs:label>ekm_connection_key_path</rdfs:label>
    <rdfs:comment>The path to the external key material on the EKM when using EkmConnection e.g., "v0/my/key". Set this field instead of externalKeyUri when using an EkmConnection.</rdfs:comment>
    <rdfs:domain rdf:resource="http://example.org/onto/class/google_kms_crypto_key_version"/>
    <rdfs:range rdf:resource="http://www.w3.org/2001/XMLSchema#string"/>
  </owl:DatatypeProperty>
  <owl:DatatypeProperty rdf:about="http://example.org/onto/prop/google_kms_crypto_key_version_external_key_uri">
    <rdfs:label>external_key_uri</rdfs:label>
    <rdfs:comment>The URI for an external resource that this CryptoKeyVersion represents.</rdfs:comment>
    <rdfs:domain rdf:resource="http://example.org/onto/class/google_kms_crypto_key_version"/>
    <rdfs:range rdf:resource="http://www.w3.org/2001/XMLSchema#string"/>
  </owl:DatatypeProperty>
  <owl:DatatypeProperty rdf:about="http://example.org/onto/prop/google_kms_crypto_key_version_create">
    <rdfs:label>create</rdfs:label>
    <rdfs:domain rdf:resource="http://example.org/onto/class/google_kms_crypto_key_version"/>
    <rdfs:range rdf:resource="http://www.w3.org/2001/XMLSchema#string"/>
  </owl:DatatypeProperty>
  <owl:DatatypeProperty rdf:about="http://example.org/onto/prop/google_kms_crypto_key_version_delete">
    <rdfs:label>delete</rdfs:label>
    <rdfs:domain rdf:resource="http://example.org/onto/class/google_kms_crypto_key_version"/>
    <rdfs:range rdf:resource="http://www.w3.org/2001/XMLSchema#string"/>
  </owl:DatatypeProperty>
  <owl:DatatypeProperty rdf:about="http://example.org/onto/prop/google_kms_crypto_key_version_update">
    <rdfs:label>update</rdfs:label>
    <rdfs:domain rdf:resource="http://example.org/onto/class/google_kms_crypto_key_version"/>
    <rdfs:range rdf:resource="http://www.w3.org/2001/XMLSchema#string"/>
  </owl:DatatypeProperty>
</rdf:RDF>
