<?xml version="1.0" encoding="UTF-8"?>
<rdf:RDF
  xmlns:rdf="http://www.w3.org/1999/02/22-rdf-syntax-ns#"
  xmlns:rdfs="http://www.w3.org/2000/01/rdf-schema#"
  xmlns:owl="http://www.w3.org/2002/07/owl#"
  xmlns:xsd="http://www.w3.org/2001/XMLSchema#"
  xml:base="http://example.org/onto/">
  <owl:Class rdf:about="http://example.org/onto/class/google_access_context_manager_authorized_orgs_desc">
    <rdfs:label>google_access_context_manager_authorized_orgs_desc</rdfs:label>
    <rdfs:comment>#
#     ***     AUTO GENERATED CODE    ***    Type: MMv1     ***
#
# ----------------------------------------------------------------------------
#
#     This code is generated by Magic Modules using the following:
#
#     Configuration: https:#github.com/GoogleCloudPlatform/magic-modules/tree/main/mmv1/products/accesscontextmanager/AuthorizedOrgsDesc.yaml
#     Template:      https:#github.com/GoogleCloudPlatform/magic-modules/tree/main/mmv1/templates/terraform/resource.html.markdown.tmpl
#
#     DO NOT EDIT this file directly. Any changes made to this file will be
#     overwritten during the next generation cycle.
#
# ----------------------------------------------------------------------------
subcategory: "Access Context Manager (VPC Service Controls)"
description: |-
  An authorized organizations description describes a list of organizations
  (1) that have been authorized to use certain asset (for example, device) data
  owned by different organizations at the enforcement points, or (2) with certain
  asset (for example, device) have been authorized to access the resources in
  another organization at the enforcement points.
---</rdfs:comment>
  </owl:Class>
  <owl:DatatypeProperty rdf:about="http://example.org/onto/prop/google_access_context_manager_authorized_orgs_desc_asset_type">
    <rdfs:label>asset_type</rdfs:label>
    <rdfs:comment>The type of entities that need to use the authorization relationship during
evaluation, such as a device. Valid values are "ASSET_TYPE_DEVICE" and
"ASSET_TYPE_CREDENTIAL_STRENGTH". Possible values: ["ASSET_TYPE_DEVICE", "ASSET_TYPE_CREDENTIAL_STRENGTH"]</rdfs:comment>
    <rdfs:domain rdf:resource="http://example.org/onto/class/google_access_context_manager_authorized_orgs_desc"/>
    <rdfs:range rdf:resource="http://www.w3.org/2001/XMLSchema#string"/>
  </owl:DatatypeProperty>
  <owl:DatatypeProperty rdf:about="http://example.org/onto/prop/google_access_context_manager_authorized_orgs_desc_authorization_direction">
    <rdfs:label>authorization_direction</rdfs:label>
    <rdfs:comment>The direction of the authorization relationship between this organization
and the organizations listed in the "orgs" field. The valid values for this
field include the following:

AUTHORIZATION_DIRECTION_FROM: Allows this organization to evaluate traffic
in the organizations listed in the 'orgs' field.

AUTHORIZATION_DIRECTION_TO: Allows the organizations listed in the 'orgs'
field to evaluate the traffic in this organization.

For the authorization relationship to take effect, all of the organizations
must authorize and specify the appropriate relationship direction. For
example, if organization A authorized organization B and C to evaluate its
traffic, by specifying "AUTHORIZATION_DIRECTION_TO" as the authorization
direction, organizations B and C must specify
"AUTHORIZATION_DIRECTION_FROM" as the authorization direction in their
"AuthorizedOrgsDesc" resource. Possible values: ["AUTHORIZATION_DIRECTION_TO", "AUTHORIZATION_DIRECTION_FROM"]</rdfs:comment>
    <rdfs:domain rdf:resource="http://example.org/onto/class/google_access_context_manager_authorized_orgs_desc"/>
    <rdfs:range rdf:resource="http://www.w3.org/2001/XMLSchema#string"/>
  </owl:DatatypeProperty>
  <owl:DatatypeProperty rdf:about="http://example.org/onto/prop/google_access_context_manager_authorized_orgs_desc_authorization_type">
    <rdfs:label>authorization_type</rdfs:label>
    <rdfs:comment>A granular control type for authorization levels. Valid value is "AUTHORIZATION_TYPE_TRUST". Possible values: ["AUTHORIZATION_TYPE_TRUST"]</rdfs:comment>
    <rdfs:domain rdf:resource="http://example.org/onto/class/google_access_context_manager_authorized_orgs_desc"/>
    <rdfs:range rdf:resource="http://www.w3.org/2001/XMLSchema#string"/>
  </owl:DatatypeProperty>
  <owl:DatatypeProperty rdf:about="http://example.org/onto/prop/google_access_context_manager_authorized_orgs_desc_create_time">
    <rdfs:label>create_time</rdfs:label>
    <rdfs:comment>Time the AuthorizedOrgsDesc was created in UTC.</rdfs:comment>
    <rdfs:domain rdf:resource="http://example.org/onto/class/google_access_context_manager_authorized_orgs_desc"/>
    <rdfs:range rdf:resource="http://www.w3.org/2001/XMLSchema#string"/>
  </owl:DatatypeProperty>
  <owl:DatatypeProperty rdf:about="http://example.org/onto/prop/google_access_context_manager_authorized_orgs_desc_id">
    <rdfs:label>id</rdfs:label>
    <rdfs:domain rdf:resource="http://example.org/onto/class/google_access_context_manager_authorized_orgs_desc"/>
    <rdfs:range rdf:resource="http://www.w3.org/2001/XMLSchema#string"/>
  </owl:DatatypeProperty>
  <owl:DatatypeProperty rdf:about="http://example.org/onto/prop/google_access_context_manager_authorized_orgs_desc_name">
    <rdfs:label>name</rdfs:label>
    <rdfs:comment>Resource name for the 'AuthorizedOrgsDesc'. Format:
'accessPolicies/{access_policy}/authorizedOrgsDescs/{authorized_orgs_desc}'.
The 'authorized_orgs_desc' component must begin with a letter, followed by
alphanumeric characters or '_'.
After you create an 'AuthorizedOrgsDesc', you cannot change its 'name'.</rdfs:comment>
    <rdfs:domain rdf:resource="http://example.org/onto/class/google_access_context_manager_authorized_orgs_desc"/>
    <rdfs:range rdf:resource="http://www.w3.org/2001/XMLSchema#string"/>
  </owl:DatatypeProperty>
  <owl:DatatypeProperty rdf:about="http://example.org/onto/prop/google_access_context_manager_authorized_orgs_desc_orgs">
    <rdfs:label>orgs</rdfs:label>
    <rdfs:comment>The list of organization ids in this AuthorizedOrgsDesc.
Format: 'organizations/<org_number>'
Example: 'organizations/123456'</rdfs:comment>
    <rdfs:domain rdf:resource="http://example.org/onto/class/google_access_context_manager_authorized_orgs_desc"/>
    <rdfs:range rdf:resource="http://www.w3.org/2001/XMLSchema#string"/>
  </owl:DatatypeProperty>
  <owl:DatatypeProperty rdf:about="http://example.org/onto/prop/google_access_context_manager_authorized_orgs_desc_parent">
    <rdfs:label>parent</rdfs:label>
    <rdfs:comment>Required. Resource name for the access policy which owns this 'AuthorizedOrgsDesc'.</rdfs:comment>
    <rdfs:domain rdf:resource="http://example.org/onto/class/google_access_context_manager_authorized_orgs_desc"/>
    <rdfs:range rdf:resource="http://www.w3.org/2001/XMLSchema#string"/>
  </owl:DatatypeProperty>
  <owl:DatatypeProperty rdf:about="http://example.org/onto/prop/google_access_context_manager_authorized_orgs_desc_update_time">
    <rdfs:label>update_time</rdfs:label>
    <rdfs:comment>Time the AuthorizedOrgsDesc was updated in UTC.</rdfs:comment>
    <rdfs:domain rdf:resource="http://example.org/onto/class/google_access_context_manager_authorized_orgs_desc"/>
    <rdfs:range rdf:resource="http://www.w3.org/2001/XMLSchema#string"/>
  </owl:DatatypeProperty>
  <owl:DatatypeProperty rdf:about="http://example.org/onto/prop/google_access_context_manager_authorized_orgs_desc_create">
    <rdfs:label>create</rdfs:label>
    <rdfs:domain rdf:resource="http://example.org/onto/class/google_access_context_manager_authorized_orgs_desc"/>
    <rdfs:range rdf:resource="http://www.w3.org/2001/XMLSchema#string"/>
  </owl:DatatypeProperty>
  <owl:DatatypeProperty rdf:about="http://example.org/onto/prop/google_access_context_manager_authorized_orgs_desc_delete">
    <rdfs:label>delete</rdfs:label>
    <rdfs:domain rdf:resource="http://example.org/onto/class/google_access_context_manager_authorized_orgs_desc"/>
    <rdfs:range rdf:resource="http://www.w3.org/2001/XMLSchema#string"/>
  </owl:DatatypeProperty>
  <owl:DatatypeProperty rdf:about="http://example.org/onto/prop/google_access_context_manager_authorized_orgs_desc_update">
    <rdfs:label>update</rdfs:label>
    <rdfs:domain rdf:resource="http://example.org/onto/class/google_access_context_manager_authorized_orgs_desc"/>
    <rdfs:range rdf:resource="http://www.w3.org/2001/XMLSchema#string"/>
  </owl:DatatypeProperty>
</rdf:RDF>
