<?xml version="1.0" encoding="UTF-8"?>
<rdf:RDF
  xmlns:rdf="http://www.w3.org/1999/02/22-rdf-syntax-ns#"
  xmlns:rdfs="http://www.w3.org/2000/01/rdf-schema#"
  xmlns:owl="http://www.w3.org/2002/07/owl#"
  xmlns:xsd="http://www.w3.org/2001/XMLSchema#"
  xml:base="http://example.org/onto/">
  <owl:Class rdf:about="http://example.org/onto/class/google_compute_vpn_tunnel">
    <rdfs:label>google_compute_vpn_tunnel</rdfs:label>
    <rdfs:comment>#
#     ***     AUTO GENERATED CODE    ***    Type: MMv1     ***
#
# ----------------------------------------------------------------------------
#
#     This code is generated by Magic Modules using the following:
#
#     Configuration: https:#github.com/GoogleCloudPlatform/magic-modules/tree/main/mmv1/products/compute/VpnTunnel.yaml
#     Template:      https:#github.com/GoogleCloudPlatform/magic-modules/tree/main/mmv1/templates/terraform/resource.html.markdown.tmpl
#
#     DO NOT EDIT this file directly. Any changes made to this file will be
#     overwritten during the next generation cycle.
#
# ----------------------------------------------------------------------------
subcategory: "Compute Engine"
description: |-
  VPN tunnel resource.
---</rdfs:comment>
  </owl:Class>
  <owl:DatatypeProperty rdf:about="http://example.org/onto/prop/google_compute_vpn_tunnel_creation_timestamp">
    <rdfs:label>creation_timestamp</rdfs:label>
    <rdfs:comment>Creation timestamp in RFC3339 text format.</rdfs:comment>
    <rdfs:domain rdf:resource="http://example.org/onto/class/google_compute_vpn_tunnel"/>
    <rdfs:range rdf:resource="http://www.w3.org/2001/XMLSchema#string"/>
  </owl:DatatypeProperty>
  <owl:DatatypeProperty rdf:about="http://example.org/onto/prop/google_compute_vpn_tunnel_description">
    <rdfs:label>description</rdfs:label>
    <rdfs:comment>An optional description of this resource.</rdfs:comment>
    <rdfs:domain rdf:resource="http://example.org/onto/class/google_compute_vpn_tunnel"/>
    <rdfs:range rdf:resource="http://www.w3.org/2001/XMLSchema#string"/>
  </owl:DatatypeProperty>
  <owl:DatatypeProperty rdf:about="http://example.org/onto/prop/google_compute_vpn_tunnel_detailed_status">
    <rdfs:label>detailed_status</rdfs:label>
    <rdfs:comment>Detailed status message for the VPN tunnel.</rdfs:comment>
    <rdfs:domain rdf:resource="http://example.org/onto/class/google_compute_vpn_tunnel"/>
    <rdfs:range rdf:resource="http://www.w3.org/2001/XMLSchema#string"/>
  </owl:DatatypeProperty>
  <owl:DatatypeProperty rdf:about="http://example.org/onto/prop/google_compute_vpn_tunnel_effective_labels">
    <rdfs:label>effective_labels</rdfs:label>
    <rdfs:comment>All of labels (key/value pairs) present on the resource in GCP, including the labels configured through Terraform, other clients and services.</rdfs:comment>
    <rdfs:domain rdf:resource="http://example.org/onto/class/google_compute_vpn_tunnel"/>
    <rdfs:range rdf:resource="http://www.w3.org/2001/XMLSchema#string"/>
  </owl:DatatypeProperty>
  <owl:DatatypeProperty rdf:about="http://example.org/onto/prop/google_compute_vpn_tunnel_id">
    <rdfs:label>id</rdfs:label>
    <rdfs:domain rdf:resource="http://example.org/onto/class/google_compute_vpn_tunnel"/>
    <rdfs:range rdf:resource="http://www.w3.org/2001/XMLSchema#string"/>
  </owl:DatatypeProperty>
  <owl:DatatypeProperty rdf:about="http://example.org/onto/prop/google_compute_vpn_tunnel_ike_version">
    <rdfs:label>ike_version</rdfs:label>
    <rdfs:comment>IKE protocol version to use when establishing the VPN tunnel with
peer VPN gateway.
Acceptable IKE versions are 1 or 2. Default version is 2.</rdfs:comment>
    <rdfs:domain rdf:resource="http://example.org/onto/class/google_compute_vpn_tunnel"/>
    <rdfs:range rdf:resource="http://www.w3.org/2001/XMLSchema#string"/>
  </owl:DatatypeProperty>
  <owl:DatatypeProperty rdf:about="http://example.org/onto/prop/google_compute_vpn_tunnel_label_fingerprint">
    <rdfs:label>label_fingerprint</rdfs:label>
    <rdfs:comment>The fingerprint used for optimistic locking of this resource.  Used
internally during updates.</rdfs:comment>
    <rdfs:domain rdf:resource="http://example.org/onto/class/google_compute_vpn_tunnel"/>
    <rdfs:range rdf:resource="http://www.w3.org/2001/XMLSchema#string"/>
  </owl:DatatypeProperty>
  <owl:DatatypeProperty rdf:about="http://example.org/onto/prop/google_compute_vpn_tunnel_labels">
    <rdfs:label>labels</rdfs:label>
    <rdfs:comment>Labels to apply to this VpnTunnel.

**Note**: This field is non-authoritative, and will only manage the labels present in your configuration.
Please refer to the field 'effective_labels' for all of the labels present on the resource.</rdfs:comment>
    <rdfs:domain rdf:resource="http://example.org/onto/class/google_compute_vpn_tunnel"/>
    <rdfs:range rdf:resource="http://www.w3.org/2001/XMLSchema#string"/>
  </owl:DatatypeProperty>
  <owl:DatatypeProperty rdf:about="http://example.org/onto/prop/google_compute_vpn_tunnel_local_traffic_selector">
    <rdfs:label>local_traffic_selector</rdfs:label>
    <rdfs:comment>Local traffic selector to use when establishing the VPN tunnel with
peer VPN gateway. The value should be a CIDR formatted string,
for example '192.168.0.0/16'. The ranges should be disjoint.
Only IPv4 is supported.</rdfs:comment>
    <rdfs:domain rdf:resource="http://example.org/onto/class/google_compute_vpn_tunnel"/>
    <rdfs:range rdf:resource="http://www.w3.org/2001/XMLSchema#string"/>
  </owl:DatatypeProperty>
  <owl:DatatypeProperty rdf:about="http://example.org/onto/prop/google_compute_vpn_tunnel_name">
    <rdfs:label>name</rdfs:label>
    <rdfs:comment>Name of the resource. The name must be 1-63 characters long, and
comply with RFC1035. Specifically, the name must be 1-63
characters long and match the regular expression
'[a-z]([-a-z0-9]*[a-z0-9])?' which means the first character
must be a lowercase letter, and all following characters must
be a dash, lowercase letter, or digit,
except the last character, which cannot be a dash.</rdfs:comment>
    <rdfs:domain rdf:resource="http://example.org/onto/class/google_compute_vpn_tunnel"/>
    <rdfs:range rdf:resource="http://www.w3.org/2001/XMLSchema#string"/>
  </owl:DatatypeProperty>
  <owl:DatatypeProperty rdf:about="http://example.org/onto/prop/google_compute_vpn_tunnel_peer_external_gateway">
    <rdfs:label>peer_external_gateway</rdfs:label>
    <rdfs:comment>URL of the peer side external VPN gateway to which this VPN tunnel is connected.</rdfs:comment>
    <rdfs:domain rdf:resource="http://example.org/onto/class/google_compute_vpn_tunnel"/>
    <rdfs:range rdf:resource="http://www.w3.org/2001/XMLSchema#string"/>
  </owl:DatatypeProperty>
  <owl:DatatypeProperty rdf:about="http://example.org/onto/prop/google_compute_vpn_tunnel_peer_external_gateway_interface">
    <rdfs:label>peer_external_gateway_interface</rdfs:label>
    <rdfs:comment>The interface ID of the external VPN gateway to which this VPN tunnel is connected.</rdfs:comment>
    <rdfs:domain rdf:resource="http://example.org/onto/class/google_compute_vpn_tunnel"/>
    <rdfs:range rdf:resource="http://www.w3.org/2001/XMLSchema#string"/>
  </owl:DatatypeProperty>
  <owl:DatatypeProperty rdf:about="http://example.org/onto/prop/google_compute_vpn_tunnel_peer_gcp_gateway">
    <rdfs:label>peer_gcp_gateway</rdfs:label>
    <rdfs:comment>URL of the peer side HA GCP VPN gateway to which this VPN tunnel is connected.
If provided, the VPN tunnel will automatically use the same vpn_gateway_interface
ID in the peer GCP VPN gateway.
This field must reference a 'google_compute_ha_vpn_gateway' resource.</rdfs:comment>
    <rdfs:domain rdf:resource="http://example.org/onto/class/google_compute_vpn_tunnel"/>
    <rdfs:range rdf:resource="http://www.w3.org/2001/XMLSchema#string"/>
  </owl:DatatypeProperty>
  <owl:DatatypeProperty rdf:about="http://example.org/onto/prop/google_compute_vpn_tunnel_peer_ip">
    <rdfs:label>peer_ip</rdfs:label>
    <rdfs:comment>IP address of the peer VPN gateway. Only IPv4 is supported.</rdfs:comment>
    <rdfs:domain rdf:resource="http://example.org/onto/class/google_compute_vpn_tunnel"/>
    <rdfs:range rdf:resource="http://www.w3.org/2001/XMLSchema#string"/>
  </owl:DatatypeProperty>
  <owl:DatatypeProperty rdf:about="http://example.org/onto/prop/google_compute_vpn_tunnel_project">
    <rdfs:label>project</rdfs:label>
    <rdfs:domain rdf:resource="http://example.org/onto/class/google_compute_vpn_tunnel"/>
    <rdfs:range rdf:resource="http://www.w3.org/2001/XMLSchema#string"/>
  </owl:DatatypeProperty>
  <owl:DatatypeProperty rdf:about="http://example.org/onto/prop/google_compute_vpn_tunnel_region">
    <rdfs:label>region</rdfs:label>
    <rdfs:comment>The region where the tunnel is located. If unset, is set to the region of 'target_vpn_gateway'.</rdfs:comment>
    <rdfs:domain rdf:resource="http://example.org/onto/class/google_compute_vpn_tunnel"/>
    <rdfs:range rdf:resource="http://www.w3.org/2001/XMLSchema#string"/>
  </owl:DatatypeProperty>
  <owl:DatatypeProperty rdf:about="http://example.org/onto/prop/google_compute_vpn_tunnel_remote_traffic_selector">
    <rdfs:label>remote_traffic_selector</rdfs:label>
    <rdfs:comment>Remote traffic selector to use when establishing the VPN tunnel with
peer VPN gateway. The value should be a CIDR formatted string,
for example '192.168.0.0/16'. The ranges should be disjoint.
Only IPv4 is supported.</rdfs:comment>
    <rdfs:domain rdf:resource="http://example.org/onto/class/google_compute_vpn_tunnel"/>
    <rdfs:range rdf:resource="http://www.w3.org/2001/XMLSchema#string"/>
  </owl:DatatypeProperty>
  <owl:DatatypeProperty rdf:about="http://example.org/onto/prop/google_compute_vpn_tunnel_router">
    <rdfs:label>router</rdfs:label>
    <rdfs:comment>URL of router resource to be used for dynamic routing.</rdfs:comment>
    <rdfs:domain rdf:resource="http://example.org/onto/class/google_compute_vpn_tunnel"/>
    <rdfs:range rdf:resource="http://www.w3.org/2001/XMLSchema#string"/>
  </owl:DatatypeProperty>
  <owl:DatatypeProperty rdf:about="http://example.org/onto/prop/google_compute_vpn_tunnel_self_link">
    <rdfs:label>self_link</rdfs:label>
    <rdfs:domain rdf:resource="http://example.org/onto/class/google_compute_vpn_tunnel"/>
    <rdfs:range rdf:resource="http://www.w3.org/2001/XMLSchema#string"/>
  </owl:DatatypeProperty>
  <owl:DatatypeProperty rdf:about="http://example.org/onto/prop/google_compute_vpn_tunnel_shared_secret">
    <rdfs:label>shared_secret</rdfs:label>
    <rdfs:comment>Shared secret used to set the secure session between the Cloud VPN
gateway and the peer VPN gateway.</rdfs:comment>
    <rdfs:domain rdf:resource="http://example.org/onto/class/google_compute_vpn_tunnel"/>
    <rdfs:range rdf:resource="http://www.w3.org/2001/XMLSchema#string"/>
  </owl:DatatypeProperty>
  <owl:DatatypeProperty rdf:about="http://example.org/onto/prop/google_compute_vpn_tunnel_shared_secret_hash">
    <rdfs:label>shared_secret_hash</rdfs:label>
    <rdfs:comment>Hash of the shared secret.</rdfs:comment>
    <rdfs:domain rdf:resource="http://example.org/onto/class/google_compute_vpn_tunnel"/>
    <rdfs:range rdf:resource="http://www.w3.org/2001/XMLSchema#string"/>
  </owl:DatatypeProperty>
  <owl:DatatypeProperty rdf:about="http://example.org/onto/prop/google_compute_vpn_tunnel_shared_secret_wo">
    <rdfs:label>shared_secret_wo</rdfs:label>
    <rdfs:comment>Shared secret used to set the secure session between the Cloud VPN
gateway and the peer VPN gateway.
 Note: This property is write-only and will not be read from the API. For more info see [updating write-only attributes](/docs/providers/google/guides/using_write_only_attributes.html#updating-write-only-attributes)</rdfs:comment>
    <rdfs:domain rdf:resource="http://example.org/onto/class/google_compute_vpn_tunnel"/>
    <rdfs:range rdf:resource="http://www.w3.org/2001/XMLSchema#string"/>
  </owl:DatatypeProperty>
  <owl:DatatypeProperty rdf:about="http://example.org/onto/prop/google_compute_vpn_tunnel_shared_secret_wo_version">
    <rdfs:label>shared_secret_wo_version</rdfs:label>
    <rdfs:comment>Triggers update of shared_secret_wo write-only. For more info see [updating write-only attributes](/docs/providers/google/guides/using_write_only_attributes.html#updating-write-only-attributes)</rdfs:comment>
    <rdfs:domain rdf:resource="http://example.org/onto/class/google_compute_vpn_tunnel"/>
    <rdfs:range rdf:resource="http://www.w3.org/2001/XMLSchema#string"/>
  </owl:DatatypeProperty>
  <owl:DatatypeProperty rdf:about="http://example.org/onto/prop/google_compute_vpn_tunnel_target_vpn_gateway">
    <rdfs:label>target_vpn_gateway</rdfs:label>
    <rdfs:comment>URL of the Target VPN gateway with which this VPN tunnel is
associated.</rdfs:comment>
    <rdfs:domain rdf:resource="http://example.org/onto/class/google_compute_vpn_tunnel"/>
    <rdfs:range rdf:resource="http://www.w3.org/2001/XMLSchema#string"/>
  </owl:DatatypeProperty>
  <owl:DatatypeProperty rdf:about="http://example.org/onto/prop/google_compute_vpn_tunnel_terraform_labels">
    <rdfs:label>terraform_labels</rdfs:label>
    <rdfs:comment>The combination of labels configured directly on the resource
 and default labels configured on the provider.</rdfs:comment>
    <rdfs:domain rdf:resource="http://example.org/onto/class/google_compute_vpn_tunnel"/>
    <rdfs:range rdf:resource="http://www.w3.org/2001/XMLSchema#string"/>
  </owl:DatatypeProperty>
  <owl:DatatypeProperty rdf:about="http://example.org/onto/prop/google_compute_vpn_tunnel_tunnel_id">
    <rdfs:label>tunnel_id</rdfs:label>
    <rdfs:comment>The unique identifier for the resource. This identifier is defined by the server.</rdfs:comment>
    <rdfs:domain rdf:resource="http://example.org/onto/class/google_compute_vpn_tunnel"/>
    <rdfs:range rdf:resource="http://www.w3.org/2001/XMLSchema#string"/>
  </owl:DatatypeProperty>
  <owl:DatatypeProperty rdf:about="http://example.org/onto/prop/google_compute_vpn_tunnel_vpn_gateway">
    <rdfs:label>vpn_gateway</rdfs:label>
    <rdfs:comment>URL of the VPN gateway with which this VPN tunnel is associated.
This must be used if a High Availability VPN gateway resource is created.
This field must reference a 'google_compute_ha_vpn_gateway' resource.</rdfs:comment>
    <rdfs:domain rdf:resource="http://example.org/onto/class/google_compute_vpn_tunnel"/>
    <rdfs:range rdf:resource="http://www.w3.org/2001/XMLSchema#string"/>
  </owl:DatatypeProperty>
  <owl:DatatypeProperty rdf:about="http://example.org/onto/prop/google_compute_vpn_tunnel_vpn_gateway_interface">
    <rdfs:label>vpn_gateway_interface</rdfs:label>
    <rdfs:comment>The interface ID of the VPN gateway with which this VPN tunnel is associated.</rdfs:comment>
    <rdfs:domain rdf:resource="http://example.org/onto/class/google_compute_vpn_tunnel"/>
    <rdfs:range rdf:resource="http://www.w3.org/2001/XMLSchema#string"/>
  </owl:DatatypeProperty>
  <owl:DatatypeProperty rdf:about="http://example.org/onto/prop/google_compute_vpn_tunnel_dh">
    <rdfs:label>dh</rdfs:label>
    <rdfs:comment>Diffie-Hellman groups.</rdfs:comment>
    <rdfs:domain rdf:resource="http://example.org/onto/class/google_compute_vpn_tunnel"/>
    <rdfs:range rdf:resource="http://www.w3.org/2001/XMLSchema#string"/>
  </owl:DatatypeProperty>
  <owl:DatatypeProperty rdf:about="http://example.org/onto/prop/google_compute_vpn_tunnel_encryption">
    <rdfs:label>encryption</rdfs:label>
    <rdfs:comment>Encryption algorithms.</rdfs:comment>
    <rdfs:domain rdf:resource="http://example.org/onto/class/google_compute_vpn_tunnel"/>
    <rdfs:range rdf:resource="http://www.w3.org/2001/XMLSchema#string"/>
  </owl:DatatypeProperty>
  <owl:DatatypeProperty rdf:about="http://example.org/onto/prop/google_compute_vpn_tunnel_integrity">
    <rdfs:label>integrity</rdfs:label>
    <rdfs:comment>Integrity algorithms.</rdfs:comment>
    <rdfs:domain rdf:resource="http://example.org/onto/class/google_compute_vpn_tunnel"/>
    <rdfs:range rdf:resource="http://www.w3.org/2001/XMLSchema#string"/>
  </owl:DatatypeProperty>
  <owl:DatatypeProperty rdf:about="http://example.org/onto/prop/google_compute_vpn_tunnel_prf">
    <rdfs:label>prf</rdfs:label>
    <rdfs:comment>Pseudo-random functions.</rdfs:comment>
    <rdfs:domain rdf:resource="http://example.org/onto/class/google_compute_vpn_tunnel"/>
    <rdfs:range rdf:resource="http://www.w3.org/2001/XMLSchema#string"/>
  </owl:DatatypeProperty>
  <owl:DatatypeProperty rdf:about="http://example.org/onto/prop/google_compute_vpn_tunnel_encryption">
    <rdfs:label>encryption</rdfs:label>
    <rdfs:comment>Encryption algorithms.</rdfs:comment>
    <rdfs:domain rdf:resource="http://example.org/onto/class/google_compute_vpn_tunnel"/>
    <rdfs:range rdf:resource="http://www.w3.org/2001/XMLSchema#string"/>
  </owl:DatatypeProperty>
  <owl:DatatypeProperty rdf:about="http://example.org/onto/prop/google_compute_vpn_tunnel_integrity">
    <rdfs:label>integrity</rdfs:label>
    <rdfs:comment>Integrity algorithms.</rdfs:comment>
    <rdfs:domain rdf:resource="http://example.org/onto/class/google_compute_vpn_tunnel"/>
    <rdfs:range rdf:resource="http://www.w3.org/2001/XMLSchema#string"/>
  </owl:DatatypeProperty>
  <owl:DatatypeProperty rdf:about="http://example.org/onto/prop/google_compute_vpn_tunnel_pfs">
    <rdfs:label>pfs</rdfs:label>
    <rdfs:comment>Perfect forward secrecy groups.</rdfs:comment>
    <rdfs:domain rdf:resource="http://example.org/onto/class/google_compute_vpn_tunnel"/>
    <rdfs:range rdf:resource="http://www.w3.org/2001/XMLSchema#string"/>
  </owl:DatatypeProperty>
  <owl:DatatypeProperty rdf:about="http://example.org/onto/prop/google_compute_vpn_tunnel_create">
    <rdfs:label>create</rdfs:label>
    <rdfs:domain rdf:resource="http://example.org/onto/class/google_compute_vpn_tunnel"/>
    <rdfs:range rdf:resource="http://www.w3.org/2001/XMLSchema#string"/>
  </owl:DatatypeProperty>
  <owl:DatatypeProperty rdf:about="http://example.org/onto/prop/google_compute_vpn_tunnel_delete">
    <rdfs:label>delete</rdfs:label>
    <rdfs:domain rdf:resource="http://example.org/onto/class/google_compute_vpn_tunnel"/>
    <rdfs:range rdf:resource="http://www.w3.org/2001/XMLSchema#string"/>
  </owl:DatatypeProperty>
  <owl:DatatypeProperty rdf:about="http://example.org/onto/prop/google_compute_vpn_tunnel_update">
    <rdfs:label>update</rdfs:label>
    <rdfs:domain rdf:resource="http://example.org/onto/class/google_compute_vpn_tunnel"/>
    <rdfs:range rdf:resource="http://www.w3.org/2001/XMLSchema#string"/>
  </owl:DatatypeProperty>
</rdf:RDF>
