<?xml version="1.0" encoding="UTF-8"?>
<rdf:RDF
  xmlns:rdf="http://www.w3.org/1999/02/22-rdf-syntax-ns#"
  xmlns:rdfs="http://www.w3.org/2000/01/rdf-schema#"
  xmlns:owl="http://www.w3.org/2002/07/owl#"
  xmlns:xsd="http://www.w3.org/2001/XMLSchema#"
  xml:base="http://example.org/onto/">
  <owl:Class rdf:about="http://example.org/onto/class/google_eventarc_message_bus">
    <rdfs:label>google_eventarc_message_bus</rdfs:label>
    <rdfs:comment>#
#     ***     AUTO GENERATED CODE    ***    Type: MMv1     ***
#
# ----------------------------------------------------------------------------
#
#     This code is generated by Magic Modules using the following:
#
#     Configuration: https:#github.com/GoogleCloudPlatform/magic-modules/tree/main/mmv1/products/eventarc/MessageBus.yaml
#     Template:      https:#github.com/GoogleCloudPlatform/magic-modules/tree/main/mmv1/templates/terraform/resource.html.markdown.tmpl
#
#     DO NOT EDIT this file directly. Any changes made to this file will be
#     overwritten during the next generation cycle.
#
# ----------------------------------------------------------------------------
subcategory: "Eventarc"
description: |-
  The Eventarc MessageBus resource
---</rdfs:comment>
  </owl:Class>
  <owl:DatatypeProperty rdf:about="http://example.org/onto/prop/google_eventarc_message_bus_annotations">
    <rdfs:label>annotations</rdfs:label>
    <rdfs:comment>Optional. Resource annotations.

**Note**: This field is non-authoritative, and will only manage the annotations present in your configuration.
Please refer to the field 'effective_annotations' for all of the annotations present on the resource.</rdfs:comment>
    <rdfs:domain rdf:resource="http://example.org/onto/class/google_eventarc_message_bus"/>
    <rdfs:range rdf:resource="http://www.w3.org/2001/XMLSchema#string"/>
  </owl:DatatypeProperty>
  <owl:DatatypeProperty rdf:about="http://example.org/onto/prop/google_eventarc_message_bus_create_time">
    <rdfs:label>create_time</rdfs:label>
    <rdfs:comment>Output only. The creation time.</rdfs:comment>
    <rdfs:domain rdf:resource="http://example.org/onto/class/google_eventarc_message_bus"/>
    <rdfs:range rdf:resource="http://www.w3.org/2001/XMLSchema#string"/>
  </owl:DatatypeProperty>
  <owl:DatatypeProperty rdf:about="http://example.org/onto/prop/google_eventarc_message_bus_crypto_key_name">
    <rdfs:label>crypto_key_name</rdfs:label>
    <rdfs:comment>Optional. Resource name of a KMS crypto key (managed by the user) used to
encrypt/decrypt their event data.

It must match the pattern
'projects/*/locations/*/keyRings/*/cryptoKeys/*'.</rdfs:comment>
    <rdfs:domain rdf:resource="http://example.org/onto/class/google_eventarc_message_bus"/>
    <rdfs:range rdf:resource="http://www.w3.org/2001/XMLSchema#string"/>
  </owl:DatatypeProperty>
  <owl:DatatypeProperty rdf:about="http://example.org/onto/prop/google_eventarc_message_bus_display_name">
    <rdfs:label>display_name</rdfs:label>
    <rdfs:comment>Optional. Resource display name.</rdfs:comment>
    <rdfs:domain rdf:resource="http://example.org/onto/class/google_eventarc_message_bus"/>
    <rdfs:range rdf:resource="http://www.w3.org/2001/XMLSchema#string"/>
  </owl:DatatypeProperty>
  <owl:DatatypeProperty rdf:about="http://example.org/onto/prop/google_eventarc_message_bus_effective_annotations">
    <rdfs:label>effective_annotations</rdfs:label>
    <rdfs:comment>All of annotations (key/value pairs) present on the resource in GCP, including the annotations configured through Terraform, other clients and services.</rdfs:comment>
    <rdfs:domain rdf:resource="http://example.org/onto/class/google_eventarc_message_bus"/>
    <rdfs:range rdf:resource="http://www.w3.org/2001/XMLSchema#string"/>
  </owl:DatatypeProperty>
  <owl:DatatypeProperty rdf:about="http://example.org/onto/prop/google_eventarc_message_bus_effective_labels">
    <rdfs:label>effective_labels</rdfs:label>
    <rdfs:comment>All of labels (key/value pairs) present on the resource in GCP, including the labels configured through Terraform, other clients and services.</rdfs:comment>
    <rdfs:domain rdf:resource="http://example.org/onto/class/google_eventarc_message_bus"/>
    <rdfs:range rdf:resource="http://www.w3.org/2001/XMLSchema#string"/>
  </owl:DatatypeProperty>
  <owl:DatatypeProperty rdf:about="http://example.org/onto/prop/google_eventarc_message_bus_etag">
    <rdfs:label>etag</rdfs:label>
    <rdfs:comment>Output only. This checksum is computed by the server based on the value of other
fields, and might be sent only on update and delete requests to ensure that
the client has an up-to-date value before proceeding.</rdfs:comment>
    <rdfs:domain rdf:resource="http://example.org/onto/class/google_eventarc_message_bus"/>
    <rdfs:range rdf:resource="http://www.w3.org/2001/XMLSchema#string"/>
  </owl:DatatypeProperty>
  <owl:DatatypeProperty rdf:about="http://example.org/onto/prop/google_eventarc_message_bus_id">
    <rdfs:label>id</rdfs:label>
    <rdfs:domain rdf:resource="http://example.org/onto/class/google_eventarc_message_bus"/>
    <rdfs:range rdf:resource="http://www.w3.org/2001/XMLSchema#string"/>
  </owl:DatatypeProperty>
  <owl:DatatypeProperty rdf:about="http://example.org/onto/prop/google_eventarc_message_bus_labels">
    <rdfs:label>labels</rdfs:label>
    <rdfs:comment>Optional. Resource labels.

**Note**: This field is non-authoritative, and will only manage the labels present in your configuration.
Please refer to the field 'effective_labels' for all of the labels present on the resource.</rdfs:comment>
    <rdfs:domain rdf:resource="http://example.org/onto/class/google_eventarc_message_bus"/>
    <rdfs:range rdf:resource="http://www.w3.org/2001/XMLSchema#string"/>
  </owl:DatatypeProperty>
  <owl:DatatypeProperty rdf:about="http://example.org/onto/prop/google_eventarc_message_bus_location">
    <rdfs:label>location</rdfs:label>
    <rdfs:comment>Resource ID segment making up resource 'name'. It identifies the resource within its parent collection as described in https://google.aip.dev/122.</rdfs:comment>
    <rdfs:domain rdf:resource="http://example.org/onto/class/google_eventarc_message_bus"/>
    <rdfs:range rdf:resource="http://www.w3.org/2001/XMLSchema#string"/>
  </owl:DatatypeProperty>
  <owl:DatatypeProperty rdf:about="http://example.org/onto/prop/google_eventarc_message_bus_message_bus_id">
    <rdfs:label>message_bus_id</rdfs:label>
    <rdfs:comment>Required. The user-provided ID to be assigned to the MessageBus. It should match the
format '^[a-z]([a-z0-9-]{0,61}[a-z0-9])?$'.</rdfs:comment>
    <rdfs:domain rdf:resource="http://example.org/onto/class/google_eventarc_message_bus"/>
    <rdfs:range rdf:resource="http://www.w3.org/2001/XMLSchema#string"/>
  </owl:DatatypeProperty>
  <owl:DatatypeProperty rdf:about="http://example.org/onto/prop/google_eventarc_message_bus_name">
    <rdfs:label>name</rdfs:label>
    <rdfs:comment>Identifier. Resource name of the form
projects/{project}/locations/{location}/messageBuses/{message_bus}</rdfs:comment>
    <rdfs:domain rdf:resource="http://example.org/onto/class/google_eventarc_message_bus"/>
    <rdfs:range rdf:resource="http://www.w3.org/2001/XMLSchema#string"/>
  </owl:DatatypeProperty>
  <owl:DatatypeProperty rdf:about="http://example.org/onto/prop/google_eventarc_message_bus_project">
    <rdfs:label>project</rdfs:label>
    <rdfs:domain rdf:resource="http://example.org/onto/class/google_eventarc_message_bus"/>
    <rdfs:range rdf:resource="http://www.w3.org/2001/XMLSchema#string"/>
  </owl:DatatypeProperty>
  <owl:DatatypeProperty rdf:about="http://example.org/onto/prop/google_eventarc_message_bus_terraform_labels">
    <rdfs:label>terraform_labels</rdfs:label>
    <rdfs:comment>The combination of labels configured directly on the resource
 and default labels configured on the provider.</rdfs:comment>
    <rdfs:domain rdf:resource="http://example.org/onto/class/google_eventarc_message_bus"/>
    <rdfs:range rdf:resource="http://www.w3.org/2001/XMLSchema#string"/>
  </owl:DatatypeProperty>
  <owl:DatatypeProperty rdf:about="http://example.org/onto/prop/google_eventarc_message_bus_uid">
    <rdfs:label>uid</rdfs:label>
    <rdfs:comment>Output only. Server assigned unique identifier for the channel. The value is a UUID4
string and guaranteed to remain unchanged until the resource is deleted.</rdfs:comment>
    <rdfs:domain rdf:resource="http://example.org/onto/class/google_eventarc_message_bus"/>
    <rdfs:range rdf:resource="http://www.w3.org/2001/XMLSchema#string"/>
  </owl:DatatypeProperty>
  <owl:DatatypeProperty rdf:about="http://example.org/onto/prop/google_eventarc_message_bus_update_time">
    <rdfs:label>update_time</rdfs:label>
    <rdfs:comment>Output only. The last-modified time.</rdfs:comment>
    <rdfs:domain rdf:resource="http://example.org/onto/class/google_eventarc_message_bus"/>
    <rdfs:range rdf:resource="http://www.w3.org/2001/XMLSchema#string"/>
  </owl:DatatypeProperty>
  <owl:DatatypeProperty rdf:about="http://example.org/onto/prop/google_eventarc_message_bus_log_severity">
    <rdfs:label>log_severity</rdfs:label>
    <rdfs:comment>Optional. The minimum severity of logs that will be sent to Stackdriver/Platform
Telemetry. Logs at severitiy â‰¥ this value will be sent, unless it is NONE. Possible values: ["NONE", "DEBUG", "INFO", "NOTICE", "WARNING", "ERROR", "CRITICAL", "ALERT", "EMERGENCY"]</rdfs:comment>
    <rdfs:domain rdf:resource="http://example.org/onto/class/google_eventarc_message_bus"/>
    <rdfs:range rdf:resource="http://www.w3.org/2001/XMLSchema#string"/>
  </owl:DatatypeProperty>
  <owl:DatatypeProperty rdf:about="http://example.org/onto/prop/google_eventarc_message_bus_create">
    <rdfs:label>create</rdfs:label>
    <rdfs:domain rdf:resource="http://example.org/onto/class/google_eventarc_message_bus"/>
    <rdfs:range rdf:resource="http://www.w3.org/2001/XMLSchema#string"/>
  </owl:DatatypeProperty>
  <owl:DatatypeProperty rdf:about="http://example.org/onto/prop/google_eventarc_message_bus_delete">
    <rdfs:label>delete</rdfs:label>
    <rdfs:domain rdf:resource="http://example.org/onto/class/google_eventarc_message_bus"/>
    <rdfs:range rdf:resource="http://www.w3.org/2001/XMLSchema#string"/>
  </owl:DatatypeProperty>
  <owl:DatatypeProperty rdf:about="http://example.org/onto/prop/google_eventarc_message_bus_update">
    <rdfs:label>update</rdfs:label>
    <rdfs:domain rdf:resource="http://example.org/onto/class/google_eventarc_message_bus"/>
    <rdfs:range rdf:resource="http://www.w3.org/2001/XMLSchema#string"/>
  </owl:DatatypeProperty>
</rdf:RDF>
