<?xml version="1.0" encoding="UTF-8"?>
<rdf:RDF
  xmlns:rdf="http://www.w3.org/1999/02/22-rdf-syntax-ns#"
  xmlns:rdfs="http://www.w3.org/2000/01/rdf-schema#"
  xmlns:owl="http://www.w3.org/2002/07/owl#"
  xmlns:xsd="http://www.w3.org/2001/XMLSchema#"
  xml:base="http://example.org/onto/">
  <owl:Class rdf:about="http://example.org/onto/class/google_compute_network_attachment">
    <rdfs:label>google_compute_network_attachment</rdfs:label>
    <rdfs:comment>#
#     ***     AUTO GENERATED CODE    ***    Type: MMv1     ***
#
# ----------------------------------------------------------------------------
#
#     This code is generated by Magic Modules using the following:
#
#     Configuration: https:#github.com/GoogleCloudPlatform/magic-modules/tree/main/mmv1/products/compute/NetworkAttachment.yaml
#     Template:      https:#github.com/GoogleCloudPlatform/magic-modules/tree/main/mmv1/templates/terraform/resource.html.markdown.tmpl
#
#     DO NOT EDIT this file directly. Any changes made to this file will be
#     overwritten during the next generation cycle.
#
# ----------------------------------------------------------------------------
subcategory: "Compute Engine"
description: |-
  A network attachment is a resource that lets a producer Virtual Private Cloud (VPC) network initiate connections to a consumer VPC network through a Private Service Connect interface.
---</rdfs:comment>
  </owl:Class>
  <owl:DatatypeProperty rdf:about="http://example.org/onto/prop/google_compute_network_attachment_connection_endpoints">
    <rdfs:label>connection_endpoints</rdfs:label>
    <rdfs:comment>An array of connections for all the producers connected to this network attachment.</rdfs:comment>
    <rdfs:domain rdf:resource="http://example.org/onto/class/google_compute_network_attachment"/>
    <rdfs:range rdf:resource="http://www.w3.org/2001/XMLSchema#string"/>
  </owl:DatatypeProperty>
  <owl:DatatypeProperty rdf:about="http://example.org/onto/prop/google_compute_network_attachment_connection_preference">
    <rdfs:label>connection_preference</rdfs:label>
    <rdfs:comment>The connection preference of service attachment. The value can be set to ACCEPT_AUTOMATIC. An ACCEPT_AUTOMATIC service attachment is one that always accepts the connection from consumer forwarding rules. Possible values: ["ACCEPT_AUTOMATIC", "ACCEPT_MANUAL", "INVALID"]</rdfs:comment>
    <rdfs:domain rdf:resource="http://example.org/onto/class/google_compute_network_attachment"/>
    <rdfs:range rdf:resource="http://www.w3.org/2001/XMLSchema#string"/>
  </owl:DatatypeProperty>
  <owl:DatatypeProperty rdf:about="http://example.org/onto/prop/google_compute_network_attachment_creation_timestamp">
    <rdfs:label>creation_timestamp</rdfs:label>
    <rdfs:comment>Creation timestamp in RFC3339 text format.</rdfs:comment>
    <rdfs:domain rdf:resource="http://example.org/onto/class/google_compute_network_attachment"/>
    <rdfs:range rdf:resource="http://www.w3.org/2001/XMLSchema#string"/>
  </owl:DatatypeProperty>
  <owl:DatatypeProperty rdf:about="http://example.org/onto/prop/google_compute_network_attachment_description">
    <rdfs:label>description</rdfs:label>
    <rdfs:comment>An optional description of this resource. Provide this property when you create the resource.</rdfs:comment>
    <rdfs:domain rdf:resource="http://example.org/onto/class/google_compute_network_attachment"/>
    <rdfs:range rdf:resource="http://www.w3.org/2001/XMLSchema#string"/>
  </owl:DatatypeProperty>
  <owl:DatatypeProperty rdf:about="http://example.org/onto/prop/google_compute_network_attachment_fingerprint">
    <rdfs:label>fingerprint</rdfs:label>
    <rdfs:comment>Fingerprint of this resource. A hash of the contents stored in this object. This
field is used in optimistic locking. An up-to-date fingerprint must be provided in order to patch.</rdfs:comment>
    <rdfs:domain rdf:resource="http://example.org/onto/class/google_compute_network_attachment"/>
    <rdfs:range rdf:resource="http://www.w3.org/2001/XMLSchema#string"/>
  </owl:DatatypeProperty>
  <owl:DatatypeProperty rdf:about="http://example.org/onto/prop/google_compute_network_attachment_id">
    <rdfs:label>id</rdfs:label>
    <rdfs:comment>The unique identifier for the resource type. The server generates this identifier.</rdfs:comment>
    <rdfs:domain rdf:resource="http://example.org/onto/class/google_compute_network_attachment"/>
    <rdfs:range rdf:resource="http://www.w3.org/2001/XMLSchema#string"/>
  </owl:DatatypeProperty>
  <owl:DatatypeProperty rdf:about="http://example.org/onto/prop/google_compute_network_attachment_kind">
    <rdfs:label>kind</rdfs:label>
    <rdfs:comment>Type of the resource.</rdfs:comment>
    <rdfs:domain rdf:resource="http://example.org/onto/class/google_compute_network_attachment"/>
    <rdfs:range rdf:resource="http://www.w3.org/2001/XMLSchema#string"/>
  </owl:DatatypeProperty>
  <owl:DatatypeProperty rdf:about="http://example.org/onto/prop/google_compute_network_attachment_name">
    <rdfs:label>name</rdfs:label>
    <rdfs:comment>Name of the resource. Provided by the client when the resource is created. The name must be 1-63 characters long, and comply with RFC1035. Specifically, the name must be 1-63 characters long and match the regular expression [a-z]([-a-z0-9]*[a-z0-9])? which means the first character must be a lowercase letter, and all following characters must be a dash, lowercase letter, or digit, except the last character, which cannot be a dash.</rdfs:comment>
    <rdfs:domain rdf:resource="http://example.org/onto/class/google_compute_network_attachment"/>
    <rdfs:range rdf:resource="http://www.w3.org/2001/XMLSchema#string"/>
  </owl:DatatypeProperty>
  <owl:DatatypeProperty rdf:about="http://example.org/onto/prop/google_compute_network_attachment_network">
    <rdfs:label>network</rdfs:label>
    <rdfs:comment>The URL of the network which the Network Attachment belongs to. Practically it is inferred by fetching the network of the first subnetwork associated.
Because it is required that all the subnetworks must be from the same network, it is assured that the Network Attachment belongs to the same network as all the subnetworks.</rdfs:comment>
    <rdfs:domain rdf:resource="http://example.org/onto/class/google_compute_network_attachment"/>
    <rdfs:range rdf:resource="http://www.w3.org/2001/XMLSchema#string"/>
  </owl:DatatypeProperty>
  <owl:DatatypeProperty rdf:about="http://example.org/onto/prop/google_compute_network_attachment_producer_accept_lists">
    <rdfs:label>producer_accept_lists</rdfs:label>
    <rdfs:comment>Projects that are allowed to connect to this network attachment. The project can be specified using its id or number.</rdfs:comment>
    <rdfs:domain rdf:resource="http://example.org/onto/class/google_compute_network_attachment"/>
    <rdfs:range rdf:resource="http://www.w3.org/2001/XMLSchema#string"/>
  </owl:DatatypeProperty>
  <owl:DatatypeProperty rdf:about="http://example.org/onto/prop/google_compute_network_attachment_producer_reject_lists">
    <rdfs:label>producer_reject_lists</rdfs:label>
    <rdfs:comment>Projects that are not allowed to connect to this network attachment. The project can be specified using its id or number.</rdfs:comment>
    <rdfs:domain rdf:resource="http://example.org/onto/class/google_compute_network_attachment"/>
    <rdfs:range rdf:resource="http://www.w3.org/2001/XMLSchema#string"/>
  </owl:DatatypeProperty>
  <owl:DatatypeProperty rdf:about="http://example.org/onto/prop/google_compute_network_attachment_project">
    <rdfs:label>project</rdfs:label>
    <rdfs:domain rdf:resource="http://example.org/onto/class/google_compute_network_attachment"/>
    <rdfs:range rdf:resource="http://www.w3.org/2001/XMLSchema#string"/>
  </owl:DatatypeProperty>
  <owl:DatatypeProperty rdf:about="http://example.org/onto/prop/google_compute_network_attachment_region">
    <rdfs:label>region</rdfs:label>
    <rdfs:comment>URL of the region where the network attachment resides. This field applies only to the region resource. You must specify this field as part of the HTTP request URL. It is not settable as a field in the request body.</rdfs:comment>
    <rdfs:domain rdf:resource="http://example.org/onto/class/google_compute_network_attachment"/>
    <rdfs:range rdf:resource="http://www.w3.org/2001/XMLSchema#string"/>
  </owl:DatatypeProperty>
  <owl:DatatypeProperty rdf:about="http://example.org/onto/prop/google_compute_network_attachment_self_link">
    <rdfs:label>self_link</rdfs:label>
    <rdfs:comment>Server-defined URL for the resource.</rdfs:comment>
    <rdfs:domain rdf:resource="http://example.org/onto/class/google_compute_network_attachment"/>
    <rdfs:range rdf:resource="http://www.w3.org/2001/XMLSchema#string"/>
  </owl:DatatypeProperty>
  <owl:DatatypeProperty rdf:about="http://example.org/onto/prop/google_compute_network_attachment_self_link_with_id">
    <rdfs:label>self_link_with_id</rdfs:label>
    <rdfs:comment>Server-defined URL for this resource's resource id.</rdfs:comment>
    <rdfs:domain rdf:resource="http://example.org/onto/class/google_compute_network_attachment"/>
    <rdfs:range rdf:resource="http://www.w3.org/2001/XMLSchema#string"/>
  </owl:DatatypeProperty>
  <owl:DatatypeProperty rdf:about="http://example.org/onto/prop/google_compute_network_attachment_subnetworks">
    <rdfs:label>subnetworks</rdfs:label>
    <rdfs:comment>An array of URLs where each entry is the URL of a subnet provided by the service consumer to use for endpoints in the producers that connect to this network attachment.</rdfs:comment>
    <rdfs:domain rdf:resource="http://example.org/onto/class/google_compute_network_attachment"/>
    <rdfs:range rdf:resource="http://www.w3.org/2001/XMLSchema#string"/>
  </owl:DatatypeProperty>
  <owl:DatatypeProperty rdf:about="http://example.org/onto/prop/google_compute_network_attachment_create">
    <rdfs:label>create</rdfs:label>
    <rdfs:domain rdf:resource="http://example.org/onto/class/google_compute_network_attachment"/>
    <rdfs:range rdf:resource="http://www.w3.org/2001/XMLSchema#string"/>
  </owl:DatatypeProperty>
  <owl:DatatypeProperty rdf:about="http://example.org/onto/prop/google_compute_network_attachment_delete">
    <rdfs:label>delete</rdfs:label>
    <rdfs:domain rdf:resource="http://example.org/onto/class/google_compute_network_attachment"/>
    <rdfs:range rdf:resource="http://www.w3.org/2001/XMLSchema#string"/>
  </owl:DatatypeProperty>
  <owl:DatatypeProperty rdf:about="http://example.org/onto/prop/google_compute_network_attachment_update">
    <rdfs:label>update</rdfs:label>
    <rdfs:domain rdf:resource="http://example.org/onto/class/google_compute_network_attachment"/>
    <rdfs:range rdf:resource="http://www.w3.org/2001/XMLSchema#string"/>
  </owl:DatatypeProperty>
</rdf:RDF>
