<?xml version="1.0" encoding="UTF-8"?>
<rdf:RDF
  xmlns:rdf="http://www.w3.org/1999/02/22-rdf-syntax-ns#"
  xmlns:rdfs="http://www.w3.org/2000/01/rdf-schema#"
  xmlns:owl="http://www.w3.org/2002/07/owl#"
  xmlns:xsd="http://www.w3.org/2001/XMLSchema#"
  xml:base="http://example.org/onto/">
  <owl:Class rdf:about="http://example.org/onto/class/google_dns_policy">
    <rdfs:label>google_dns_policy</rdfs:label>
    <rdfs:comment>#
#     ***     AUTO GENERATED CODE    ***    Type: MMv1     ***
#
# ----------------------------------------------------------------------------
#
#     This code is generated by Magic Modules using the following:
#
#     Configuration: https:#github.com/GoogleCloudPlatform/magic-modules/tree/main/mmv1/products/dns/Policy.yaml
#     Template:      https:#github.com/GoogleCloudPlatform/magic-modules/tree/main/mmv1/templates/terraform/resource.html.markdown.tmpl
#
#     DO NOT EDIT this file directly. Any changes made to this file will be
#     overwritten during the next generation cycle.
#
# ----------------------------------------------------------------------------
subcategory: "Cloud DNS"
description: |-
  A policy is a collection of DNS rules applied to one or more Virtual
  Private Cloud resources.
---</rdfs:comment>
  </owl:Class>
  <owl:DatatypeProperty rdf:about="http://example.org/onto/prop/google_dns_policy_description">
    <rdfs:label>description</rdfs:label>
    <rdfs:comment>A textual description field. Defaults to 'Managed by Terraform'.</rdfs:comment>
    <rdfs:domain rdf:resource="http://example.org/onto/class/google_dns_policy"/>
    <rdfs:range rdf:resource="http://www.w3.org/2001/XMLSchema#string"/>
  </owl:DatatypeProperty>
  <owl:DatatypeProperty rdf:about="http://example.org/onto/prop/google_dns_policy_enable_inbound_forwarding">
    <rdfs:label>enable_inbound_forwarding</rdfs:label>
    <rdfs:comment>Allows networks bound to this policy to receive DNS queries sent
by VMs or applications over VPN connections. When enabled, a
virtual IP address will be allocated from each of the sub-networks
that are bound to this policy.</rdfs:comment>
    <rdfs:domain rdf:resource="http://example.org/onto/class/google_dns_policy"/>
    <rdfs:range rdf:resource="http://www.w3.org/2001/XMLSchema#string"/>
  </owl:DatatypeProperty>
  <owl:DatatypeProperty rdf:about="http://example.org/onto/prop/google_dns_policy_enable_logging">
    <rdfs:label>enable_logging</rdfs:label>
    <rdfs:comment>Controls whether logging is enabled for the networks bound to this policy.
Defaults to no logging if not set.</rdfs:comment>
    <rdfs:domain rdf:resource="http://example.org/onto/class/google_dns_policy"/>
    <rdfs:range rdf:resource="http://www.w3.org/2001/XMLSchema#string"/>
  </owl:DatatypeProperty>
  <owl:DatatypeProperty rdf:about="http://example.org/onto/prop/google_dns_policy_id">
    <rdfs:label>id</rdfs:label>
    <rdfs:domain rdf:resource="http://example.org/onto/class/google_dns_policy"/>
    <rdfs:range rdf:resource="http://www.w3.org/2001/XMLSchema#string"/>
  </owl:DatatypeProperty>
  <owl:DatatypeProperty rdf:about="http://example.org/onto/prop/google_dns_policy_name">
    <rdfs:label>name</rdfs:label>
    <rdfs:comment>User assigned name for this policy.</rdfs:comment>
    <rdfs:domain rdf:resource="http://example.org/onto/class/google_dns_policy"/>
    <rdfs:range rdf:resource="http://www.w3.org/2001/XMLSchema#string"/>
  </owl:DatatypeProperty>
  <owl:DatatypeProperty rdf:about="http://example.org/onto/prop/google_dns_policy_project">
    <rdfs:label>project</rdfs:label>
    <rdfs:domain rdf:resource="http://example.org/onto/class/google_dns_policy"/>
    <rdfs:range rdf:resource="http://www.w3.org/2001/XMLSchema#string"/>
  </owl:DatatypeProperty>
  <owl:DatatypeProperty rdf:about="http://example.org/onto/prop/google_dns_policy_forwarding_path">
    <rdfs:label>forwarding_path</rdfs:label>
    <rdfs:comment>Forwarding path for this TargetNameServer. If unset or 'default' Cloud DNS will make forwarding
decision based on address ranges, i.e. RFC1918 addresses go to the VPC, Non-RFC1918 addresses go
to the Internet. When set to 'private', Cloud DNS will always send queries through VPC for this target Possible values: ["default", "private"]</rdfs:comment>
    <rdfs:domain rdf:resource="http://example.org/onto/class/google_dns_policy"/>
    <rdfs:range rdf:resource="http://www.w3.org/2001/XMLSchema#string"/>
  </owl:DatatypeProperty>
  <owl:DatatypeProperty rdf:about="http://example.org/onto/prop/google_dns_policy_ipv4_address">
    <rdfs:label>ipv4_address</rdfs:label>
    <rdfs:comment>IPv4 address to forward to.</rdfs:comment>
    <rdfs:domain rdf:resource="http://example.org/onto/class/google_dns_policy"/>
    <rdfs:range rdf:resource="http://www.w3.org/2001/XMLSchema#string"/>
  </owl:DatatypeProperty>
  <owl:DatatypeProperty rdf:about="http://example.org/onto/prop/google_dns_policy_all_queries">
    <rdfs:label>all_queries</rdfs:label>
    <rdfs:comment>Controls whether DNS64 is enabled globally at the network level.</rdfs:comment>
    <rdfs:domain rdf:resource="http://example.org/onto/class/google_dns_policy"/>
    <rdfs:range rdf:resource="http://www.w3.org/2001/XMLSchema#string"/>
  </owl:DatatypeProperty>
  <owl:DatatypeProperty rdf:about="http://example.org/onto/prop/google_dns_policy_network_url">
    <rdfs:label>network_url</rdfs:label>
    <rdfs:comment>The id or fully qualified URL of the VPC network to forward queries to.
This should be formatted like 'projects/{project}/global/networks/{network}' or
'https://www.googleapis.com/compute/v1/projects/{project}/global/networks/{network}'</rdfs:comment>
    <rdfs:domain rdf:resource="http://example.org/onto/class/google_dns_policy"/>
    <rdfs:range rdf:resource="http://www.w3.org/2001/XMLSchema#string"/>
  </owl:DatatypeProperty>
  <owl:DatatypeProperty rdf:about="http://example.org/onto/prop/google_dns_policy_create">
    <rdfs:label>create</rdfs:label>
    <rdfs:domain rdf:resource="http://example.org/onto/class/google_dns_policy"/>
    <rdfs:range rdf:resource="http://www.w3.org/2001/XMLSchema#string"/>
  </owl:DatatypeProperty>
  <owl:DatatypeProperty rdf:about="http://example.org/onto/prop/google_dns_policy_delete">
    <rdfs:label>delete</rdfs:label>
    <rdfs:domain rdf:resource="http://example.org/onto/class/google_dns_policy"/>
    <rdfs:range rdf:resource="http://www.w3.org/2001/XMLSchema#string"/>
  </owl:DatatypeProperty>
  <owl:DatatypeProperty rdf:about="http://example.org/onto/prop/google_dns_policy_update">
    <rdfs:label>update</rdfs:label>
    <rdfs:domain rdf:resource="http://example.org/onto/class/google_dns_policy"/>
    <rdfs:range rdf:resource="http://www.w3.org/2001/XMLSchema#string"/>
  </owl:DatatypeProperty>
</rdf:RDF>
