<?xml version="1.0" encoding="UTF-8"?>
<rdf:RDF
  xmlns:rdf="http://www.w3.org/1999/02/22-rdf-syntax-ns#"
  xmlns:rdfs="http://www.w3.org/2000/01/rdf-schema#"
  xmlns:owl="http://www.w3.org/2002/07/owl#"
  xmlns:xsd="http://www.w3.org/2001/XMLSchema#"
  xml:base="http://example.org/onto/">
  <owl:Class rdf:about="http://example.org/onto/class/google_dataplex_zone">
    <rdfs:label>google_dataplex_zone</rdfs:label>
    <rdfs:comment>#
#     ***     AUTO GENERATED CODE    ***    Type: DCL     ***
#
# ----------------------------------------------------------------------------
#
#     This file is managed by Magic Modules (https:#github.com/GoogleCloudPlatform/magic-modules)
#     and is based on the DCL (https:#github.com/GoogleCloudPlatform/declarative-resource-client-library).
#     Changes will need to be made to the DCL or Magic Modules instead of here.
#
#     We are not currently able to accept contributions to this file. If changes
#     are required, please file an issue at https:#github.com/hashicorp/terraform-provider-google/issues/new/choose
#
# ----------------------------------------------------------------------------
subcategory: "Dataplex"
description: |-
  The Dataplex Zone resource
---</rdfs:comment>
  </owl:Class>
  <owl:DatatypeProperty rdf:about="http://example.org/onto/prop/google_dataplex_zone_asset_status">
    <rdfs:label>asset_status</rdfs:label>
    <rdfs:comment>Output only. Aggregated status of the underlying assets of the zone.</rdfs:comment>
    <rdfs:domain rdf:resource="http://example.org/onto/class/google_dataplex_zone"/>
    <rdfs:range rdf:resource="http://www.w3.org/2001/XMLSchema#string"/>
  </owl:DatatypeProperty>
  <owl:DatatypeProperty rdf:about="http://example.org/onto/prop/google_dataplex_zone_create_time">
    <rdfs:label>create_time</rdfs:label>
    <rdfs:comment>Output only. The time when the zone was created.</rdfs:comment>
    <rdfs:domain rdf:resource="http://example.org/onto/class/google_dataplex_zone"/>
    <rdfs:range rdf:resource="http://www.w3.org/2001/XMLSchema#string"/>
  </owl:DatatypeProperty>
  <owl:DatatypeProperty rdf:about="http://example.org/onto/prop/google_dataplex_zone_description">
    <rdfs:label>description</rdfs:label>
    <rdfs:comment>Optional. Description of the zone.</rdfs:comment>
    <rdfs:domain rdf:resource="http://example.org/onto/class/google_dataplex_zone"/>
    <rdfs:range rdf:resource="http://www.w3.org/2001/XMLSchema#string"/>
  </owl:DatatypeProperty>
  <owl:DatatypeProperty rdf:about="http://example.org/onto/prop/google_dataplex_zone_display_name">
    <rdfs:label>display_name</rdfs:label>
    <rdfs:comment>Optional. User friendly display name.</rdfs:comment>
    <rdfs:domain rdf:resource="http://example.org/onto/class/google_dataplex_zone"/>
    <rdfs:range rdf:resource="http://www.w3.org/2001/XMLSchema#string"/>
  </owl:DatatypeProperty>
  <owl:DatatypeProperty rdf:about="http://example.org/onto/prop/google_dataplex_zone_effective_labels">
    <rdfs:label>effective_labels</rdfs:label>
    <rdfs:comment>All of labels (key/value pairs) present on the resource in GCP, including the labels configured through Terraform, other clients and services.</rdfs:comment>
    <rdfs:domain rdf:resource="http://example.org/onto/class/google_dataplex_zone"/>
    <rdfs:range rdf:resource="http://www.w3.org/2001/XMLSchema#string"/>
  </owl:DatatypeProperty>
  <owl:DatatypeProperty rdf:about="http://example.org/onto/prop/google_dataplex_zone_id">
    <rdfs:label>id</rdfs:label>
    <rdfs:domain rdf:resource="http://example.org/onto/class/google_dataplex_zone"/>
    <rdfs:range rdf:resource="http://www.w3.org/2001/XMLSchema#string"/>
  </owl:DatatypeProperty>
  <owl:DatatypeProperty rdf:about="http://example.org/onto/prop/google_dataplex_zone_labels">
    <rdfs:label>labels</rdfs:label>
    <rdfs:comment>Optional. User defined labels for the zone.

**Note**: This field is non-authoritative, and will only manage the labels present in your configuration.
Please refer to the field `effective_labels` for all of the labels present on the resource.</rdfs:comment>
    <rdfs:domain rdf:resource="http://example.org/onto/class/google_dataplex_zone"/>
    <rdfs:range rdf:resource="http://www.w3.org/2001/XMLSchema#string"/>
  </owl:DatatypeProperty>
  <owl:DatatypeProperty rdf:about="http://example.org/onto/prop/google_dataplex_zone_lake">
    <rdfs:label>lake</rdfs:label>
    <rdfs:comment>The lake for the resource</rdfs:comment>
    <rdfs:domain rdf:resource="http://example.org/onto/class/google_dataplex_zone"/>
    <rdfs:range rdf:resource="http://www.w3.org/2001/XMLSchema#string"/>
  </owl:DatatypeProperty>
  <owl:DatatypeProperty rdf:about="http://example.org/onto/prop/google_dataplex_zone_location">
    <rdfs:label>location</rdfs:label>
    <rdfs:comment>The location for the resource</rdfs:comment>
    <rdfs:domain rdf:resource="http://example.org/onto/class/google_dataplex_zone"/>
    <rdfs:range rdf:resource="http://www.w3.org/2001/XMLSchema#string"/>
  </owl:DatatypeProperty>
  <owl:DatatypeProperty rdf:about="http://example.org/onto/prop/google_dataplex_zone_name">
    <rdfs:label>name</rdfs:label>
    <rdfs:comment>The name of the zone.</rdfs:comment>
    <rdfs:domain rdf:resource="http://example.org/onto/class/google_dataplex_zone"/>
    <rdfs:range rdf:resource="http://www.w3.org/2001/XMLSchema#string"/>
  </owl:DatatypeProperty>
  <owl:DatatypeProperty rdf:about="http://example.org/onto/prop/google_dataplex_zone_project">
    <rdfs:label>project</rdfs:label>
    <rdfs:comment>The project for the resource</rdfs:comment>
    <rdfs:domain rdf:resource="http://example.org/onto/class/google_dataplex_zone"/>
    <rdfs:range rdf:resource="http://www.w3.org/2001/XMLSchema#string"/>
  </owl:DatatypeProperty>
  <owl:DatatypeProperty rdf:about="http://example.org/onto/prop/google_dataplex_zone_state">
    <rdfs:label>state</rdfs:label>
    <rdfs:comment>Output only. Current state of the zone. Possible values: STATE_UNSPECIFIED, ACTIVE, CREATING, DELETING, ACTION_REQUIRED</rdfs:comment>
    <rdfs:domain rdf:resource="http://example.org/onto/class/google_dataplex_zone"/>
    <rdfs:range rdf:resource="http://www.w3.org/2001/XMLSchema#string"/>
  </owl:DatatypeProperty>
  <owl:DatatypeProperty rdf:about="http://example.org/onto/prop/google_dataplex_zone_terraform_labels">
    <rdfs:label>terraform_labels</rdfs:label>
    <rdfs:comment>The combination of labels configured directly on the resource and default labels configured on the provider.</rdfs:comment>
    <rdfs:domain rdf:resource="http://example.org/onto/class/google_dataplex_zone"/>
    <rdfs:range rdf:resource="http://www.w3.org/2001/XMLSchema#string"/>
  </owl:DatatypeProperty>
  <owl:DatatypeProperty rdf:about="http://example.org/onto/prop/google_dataplex_zone_type">
    <rdfs:label>type</rdfs:label>
    <rdfs:comment>Required. Immutable. The type of the zone. Possible values: TYPE_UNSPECIFIED, RAW, CURATED</rdfs:comment>
    <rdfs:domain rdf:resource="http://example.org/onto/class/google_dataplex_zone"/>
    <rdfs:range rdf:resource="http://www.w3.org/2001/XMLSchema#string"/>
  </owl:DatatypeProperty>
  <owl:DatatypeProperty rdf:about="http://example.org/onto/prop/google_dataplex_zone_uid">
    <rdfs:label>uid</rdfs:label>
    <rdfs:comment>Output only. System generated globally unique ID for the zone. This ID will be different if the zone is deleted and re-created with the same name.</rdfs:comment>
    <rdfs:domain rdf:resource="http://example.org/onto/class/google_dataplex_zone"/>
    <rdfs:range rdf:resource="http://www.w3.org/2001/XMLSchema#string"/>
  </owl:DatatypeProperty>
  <owl:DatatypeProperty rdf:about="http://example.org/onto/prop/google_dataplex_zone_update_time">
    <rdfs:label>update_time</rdfs:label>
    <rdfs:comment>Output only. The time when the zone was last updated.</rdfs:comment>
    <rdfs:domain rdf:resource="http://example.org/onto/class/google_dataplex_zone"/>
    <rdfs:range rdf:resource="http://www.w3.org/2001/XMLSchema#string"/>
  </owl:DatatypeProperty>
  <owl:DatatypeProperty rdf:about="http://example.org/onto/prop/google_dataplex_zone_enabled">
    <rdfs:label>enabled</rdfs:label>
    <rdfs:comment>Required. Whether discovery is enabled.</rdfs:comment>
    <rdfs:domain rdf:resource="http://example.org/onto/class/google_dataplex_zone"/>
    <rdfs:range rdf:resource="http://www.w3.org/2001/XMLSchema#string"/>
  </owl:DatatypeProperty>
  <owl:DatatypeProperty rdf:about="http://example.org/onto/prop/google_dataplex_zone_exclude_patterns">
    <rdfs:label>exclude_patterns</rdfs:label>
    <rdfs:comment>Optional. The list of patterns to apply for selecting data to exclude during discovery. For Cloud Storage bucket assets, these are interpreted as glob patterns used to match object names. For BigQuery dataset assets, these are interpreted as patterns to match table names.</rdfs:comment>
    <rdfs:domain rdf:resource="http://example.org/onto/class/google_dataplex_zone"/>
    <rdfs:range rdf:resource="http://www.w3.org/2001/XMLSchema#string"/>
  </owl:DatatypeProperty>
  <owl:DatatypeProperty rdf:about="http://example.org/onto/prop/google_dataplex_zone_include_patterns">
    <rdfs:label>include_patterns</rdfs:label>
    <rdfs:comment>Optional. The list of patterns to apply for selecting data to include during discovery if only a subset of the data should considered. For Cloud Storage bucket assets, these are interpreted as glob patterns used to match object names. For BigQuery dataset assets, these are interpreted as patterns to match table names.</rdfs:comment>
    <rdfs:domain rdf:resource="http://example.org/onto/class/google_dataplex_zone"/>
    <rdfs:range rdf:resource="http://www.w3.org/2001/XMLSchema#string"/>
  </owl:DatatypeProperty>
  <owl:DatatypeProperty rdf:about="http://example.org/onto/prop/google_dataplex_zone_schedule">
    <rdfs:label>schedule</rdfs:label>
    <rdfs:comment>Optional. Cron schedule (https://en.wikipedia.org/wiki/Cron) for running discovery periodically. Successive discovery runs must be scheduled at least 60 minutes apart. The default value is to run discovery every 60 minutes. To explicitly set a timezone to the cron tab, apply a prefix in the cron tab: "CRON_TZ=${IANA_TIME_ZONE}" or TZ=${IANA_TIME_ZONE}". The ${IANA_TIME_ZONE} may only be a valid string from IANA time zone database. For example, "CRON_TZ=America/New_York 1 * * * *", or "TZ=America/New_York 1 * * * *".</rdfs:comment>
    <rdfs:domain rdf:resource="http://example.org/onto/class/google_dataplex_zone"/>
    <rdfs:range rdf:resource="http://www.w3.org/2001/XMLSchema#string"/>
  </owl:DatatypeProperty>
  <owl:DatatypeProperty rdf:about="http://example.org/onto/prop/google_dataplex_zone_delimiter">
    <rdfs:label>delimiter</rdfs:label>
    <rdfs:comment>Optional. The delimiter being used to separate values. This defaults to ','.</rdfs:comment>
    <rdfs:domain rdf:resource="http://example.org/onto/class/google_dataplex_zone"/>
    <rdfs:range rdf:resource="http://www.w3.org/2001/XMLSchema#string"/>
  </owl:DatatypeProperty>
  <owl:DatatypeProperty rdf:about="http://example.org/onto/prop/google_dataplex_zone_disable_type_inference">
    <rdfs:label>disable_type_inference</rdfs:label>
    <rdfs:comment>Optional. Whether to disable the inference of data type for CSV data. If true, all columns will be registered as strings.</rdfs:comment>
    <rdfs:domain rdf:resource="http://example.org/onto/class/google_dataplex_zone"/>
    <rdfs:range rdf:resource="http://www.w3.org/2001/XMLSchema#string"/>
  </owl:DatatypeProperty>
  <owl:DatatypeProperty rdf:about="http://example.org/onto/prop/google_dataplex_zone_encoding">
    <rdfs:label>encoding</rdfs:label>
    <rdfs:comment>Optional. The character encoding of the data. The default is UTF-8.</rdfs:comment>
    <rdfs:domain rdf:resource="http://example.org/onto/class/google_dataplex_zone"/>
    <rdfs:range rdf:resource="http://www.w3.org/2001/XMLSchema#string"/>
  </owl:DatatypeProperty>
  <owl:DatatypeProperty rdf:about="http://example.org/onto/prop/google_dataplex_zone_header_rows">
    <rdfs:label>header_rows</rdfs:label>
    <rdfs:comment>Optional. The number of rows to interpret as header rows that should be skipped when reading data rows.</rdfs:comment>
    <rdfs:domain rdf:resource="http://example.org/onto/class/google_dataplex_zone"/>
    <rdfs:range rdf:resource="http://www.w3.org/2001/XMLSchema#string"/>
  </owl:DatatypeProperty>
  <owl:DatatypeProperty rdf:about="http://example.org/onto/prop/google_dataplex_zone_disable_type_inference">
    <rdfs:label>disable_type_inference</rdfs:label>
    <rdfs:comment>Optional. Whether to disable the inference of data type for Json data. If true, all columns will be registered as their primitive types (strings, number or boolean).</rdfs:comment>
    <rdfs:domain rdf:resource="http://example.org/onto/class/google_dataplex_zone"/>
    <rdfs:range rdf:resource="http://www.w3.org/2001/XMLSchema#string"/>
  </owl:DatatypeProperty>
  <owl:DatatypeProperty rdf:about="http://example.org/onto/prop/google_dataplex_zone_encoding">
    <rdfs:label>encoding</rdfs:label>
    <rdfs:comment>Optional. The character encoding of the data. The default is UTF-8.</rdfs:comment>
    <rdfs:domain rdf:resource="http://example.org/onto/class/google_dataplex_zone"/>
    <rdfs:range rdf:resource="http://www.w3.org/2001/XMLSchema#string"/>
  </owl:DatatypeProperty>
  <owl:DatatypeProperty rdf:about="http://example.org/onto/prop/google_dataplex_zone_location_type">
    <rdfs:label>location_type</rdfs:label>
    <rdfs:comment>Required. Immutable. The location type of the resources that are allowed to be attached to the assets within this zone. Possible values: LOCATION_TYPE_UNSPECIFIED, SINGLE_REGION, MULTI_REGION</rdfs:comment>
    <rdfs:domain rdf:resource="http://example.org/onto/class/google_dataplex_zone"/>
    <rdfs:range rdf:resource="http://www.w3.org/2001/XMLSchema#string"/>
  </owl:DatatypeProperty>
  <owl:DatatypeProperty rdf:about="http://example.org/onto/prop/google_dataplex_zone_create">
    <rdfs:label>create</rdfs:label>
    <rdfs:domain rdf:resource="http://example.org/onto/class/google_dataplex_zone"/>
    <rdfs:range rdf:resource="http://www.w3.org/2001/XMLSchema#string"/>
  </owl:DatatypeProperty>
  <owl:DatatypeProperty rdf:about="http://example.org/onto/prop/google_dataplex_zone_delete">
    <rdfs:label>delete</rdfs:label>
    <rdfs:domain rdf:resource="http://example.org/onto/class/google_dataplex_zone"/>
    <rdfs:range rdf:resource="http://www.w3.org/2001/XMLSchema#string"/>
  </owl:DatatypeProperty>
  <owl:DatatypeProperty rdf:about="http://example.org/onto/prop/google_dataplex_zone_update">
    <rdfs:label>update</rdfs:label>
    <rdfs:domain rdf:resource="http://example.org/onto/class/google_dataplex_zone"/>
    <rdfs:range rdf:resource="http://www.w3.org/2001/XMLSchema#string"/>
  </owl:DatatypeProperty>
</rdf:RDF>
