<?xml version="1.0" encoding="UTF-8"?>
<rdf:RDF
  xmlns:rdf="http://www.w3.org/1999/02/22-rdf-syntax-ns#"
  xmlns:rdfs="http://www.w3.org/2000/01/rdf-schema#"
  xmlns:owl="http://www.w3.org/2002/07/owl#"
  xmlns:xsd="http://www.w3.org/2001/XMLSchema#"
  xml:base="http://example.org/onto/">
  <owl:Class rdf:about="http://example.org/onto/class/google_parameter_manager_regional_parameter_version">
    <rdfs:label>google_parameter_manager_regional_parameter_version</rdfs:label>
    <rdfs:comment>#
#     ***     AUTO GENERATED CODE    ***    Type: MMv1     ***
#
# ----------------------------------------------------------------------------
#
#     This code is generated by Magic Modules using the following:
#
#     Configuration: https:#github.com/GoogleCloudPlatform/magic-modules/tree/main/mmv1/products/parametermanagerregional/RegionalParameterVersion.yaml
#     Template:      https:#github.com/GoogleCloudPlatform/magic-modules/tree/main/mmv1/templates/terraform/resource.html.markdown.tmpl
#
#     DO NOT EDIT this file directly. Any changes made to this file will be
#     overwritten during the next generation cycle.
#
# ----------------------------------------------------------------------------
subcategory: "Parameter Manager"
description: |-
  A Regional Parameter Version resource that stores the actual value of the regional parameter.
---</rdfs:comment>
  </owl:Class>
  <owl:DatatypeProperty rdf:about="http://example.org/onto/prop/google_parameter_manager_regional_parameter_version_create_time">
    <rdfs:label>create_time</rdfs:label>
    <rdfs:comment>The time at which the Regional Parameter Version was created.</rdfs:comment>
    <rdfs:domain rdf:resource="http://example.org/onto/class/google_parameter_manager_regional_parameter_version"/>
    <rdfs:range rdf:resource="http://www.w3.org/2001/XMLSchema#string"/>
  </owl:DatatypeProperty>
  <owl:DatatypeProperty rdf:about="http://example.org/onto/prop/google_parameter_manager_regional_parameter_version_disabled">
    <rdfs:label>disabled</rdfs:label>
    <rdfs:comment>The current state of Regional Parameter Version. This field is only applicable for updating Regional Parameter Version.</rdfs:comment>
    <rdfs:domain rdf:resource="http://example.org/onto/class/google_parameter_manager_regional_parameter_version"/>
    <rdfs:range rdf:resource="http://www.w3.org/2001/XMLSchema#string"/>
  </owl:DatatypeProperty>
  <owl:DatatypeProperty rdf:about="http://example.org/onto/prop/google_parameter_manager_regional_parameter_version_id">
    <rdfs:label>id</rdfs:label>
    <rdfs:domain rdf:resource="http://example.org/onto/class/google_parameter_manager_regional_parameter_version"/>
    <rdfs:range rdf:resource="http://www.w3.org/2001/XMLSchema#string"/>
  </owl:DatatypeProperty>
  <owl:DatatypeProperty rdf:about="http://example.org/onto/prop/google_parameter_manager_regional_parameter_version_kms_key_version">
    <rdfs:label>kms_key_version</rdfs:label>
    <rdfs:comment>The resource name of the Cloud KMS CryptoKeyVersion used to decrypt regional parameter version payload. Format
'projects/{{project}}/locations/{{location}}/keyRings/{{key_ring}}/cryptoKeys/{{crypto_key}}/cryptoKeyVersions/{{crypto_key_version}}'</rdfs:comment>
    <rdfs:domain rdf:resource="http://example.org/onto/class/google_parameter_manager_regional_parameter_version"/>
    <rdfs:range rdf:resource="http://www.w3.org/2001/XMLSchema#string"/>
  </owl:DatatypeProperty>
  <owl:DatatypeProperty rdf:about="http://example.org/onto/prop/google_parameter_manager_regional_parameter_version_location">
    <rdfs:label>location</rdfs:label>
    <rdfs:comment>Location of Parameter Manager Regional parameter resource.</rdfs:comment>
    <rdfs:domain rdf:resource="http://example.org/onto/class/google_parameter_manager_regional_parameter_version"/>
    <rdfs:range rdf:resource="http://www.w3.org/2001/XMLSchema#string"/>
  </owl:DatatypeProperty>
  <owl:DatatypeProperty rdf:about="http://example.org/onto/prop/google_parameter_manager_regional_parameter_version_name">
    <rdfs:label>name</rdfs:label>
    <rdfs:comment>The resource name of the Regional Parameter Version. Format:
'projects/{{project}}/locations/{{location}}/parameters/{{parameter_id}}/versions/{{parameter_version_id}}'</rdfs:comment>
    <rdfs:domain rdf:resource="http://example.org/onto/class/google_parameter_manager_regional_parameter_version"/>
    <rdfs:range rdf:resource="http://www.w3.org/2001/XMLSchema#string"/>
  </owl:DatatypeProperty>
  <owl:DatatypeProperty rdf:about="http://example.org/onto/prop/google_parameter_manager_regional_parameter_version_parameter">
    <rdfs:label>parameter</rdfs:label>
    <rdfs:comment>Parameter Manager Regional Parameter resource.</rdfs:comment>
    <rdfs:domain rdf:resource="http://example.org/onto/class/google_parameter_manager_regional_parameter_version"/>
    <rdfs:range rdf:resource="http://www.w3.org/2001/XMLSchema#string"/>
  </owl:DatatypeProperty>
  <owl:DatatypeProperty rdf:about="http://example.org/onto/prop/google_parameter_manager_regional_parameter_version_parameter_data">
    <rdfs:label>parameter_data</rdfs:label>
    <rdfs:comment>The Regional Parameter data.</rdfs:comment>
    <rdfs:domain rdf:resource="http://example.org/onto/class/google_parameter_manager_regional_parameter_version"/>
    <rdfs:range rdf:resource="http://www.w3.org/2001/XMLSchema#string"/>
  </owl:DatatypeProperty>
  <owl:DatatypeProperty rdf:about="http://example.org/onto/prop/google_parameter_manager_regional_parameter_version_parameter_version_id">
    <rdfs:label>parameter_version_id</rdfs:label>
    <rdfs:comment>Version ID of the Regional Parameter Version Resource. This must be unique within the Regional Parameter.</rdfs:comment>
    <rdfs:domain rdf:resource="http://example.org/onto/class/google_parameter_manager_regional_parameter_version"/>
    <rdfs:range rdf:resource="http://www.w3.org/2001/XMLSchema#string"/>
  </owl:DatatypeProperty>
  <owl:DatatypeProperty rdf:about="http://example.org/onto/prop/google_parameter_manager_regional_parameter_version_update_time">
    <rdfs:label>update_time</rdfs:label>
    <rdfs:comment>The time at which the Regional Parameter Version was updated.</rdfs:comment>
    <rdfs:domain rdf:resource="http://example.org/onto/class/google_parameter_manager_regional_parameter_version"/>
    <rdfs:range rdf:resource="http://www.w3.org/2001/XMLSchema#string"/>
  </owl:DatatypeProperty>
  <owl:DatatypeProperty rdf:about="http://example.org/onto/prop/google_parameter_manager_regional_parameter_version_create">
    <rdfs:label>create</rdfs:label>
    <rdfs:domain rdf:resource="http://example.org/onto/class/google_parameter_manager_regional_parameter_version"/>
    <rdfs:range rdf:resource="http://www.w3.org/2001/XMLSchema#string"/>
  </owl:DatatypeProperty>
  <owl:DatatypeProperty rdf:about="http://example.org/onto/prop/google_parameter_manager_regional_parameter_version_delete">
    <rdfs:label>delete</rdfs:label>
    <rdfs:domain rdf:resource="http://example.org/onto/class/google_parameter_manager_regional_parameter_version"/>
    <rdfs:range rdf:resource="http://www.w3.org/2001/XMLSchema#string"/>
  </owl:DatatypeProperty>
  <owl:DatatypeProperty rdf:about="http://example.org/onto/prop/google_parameter_manager_regional_parameter_version_update">
    <rdfs:label>update</rdfs:label>
    <rdfs:domain rdf:resource="http://example.org/onto/class/google_parameter_manager_regional_parameter_version"/>
    <rdfs:range rdf:resource="http://www.w3.org/2001/XMLSchema#string"/>
  </owl:DatatypeProperty>
</rdf:RDF>
