<?xml version="1.0" encoding="UTF-8"?>
<rdf:RDF
  xmlns:rdf="http://www.w3.org/1999/02/22-rdf-syntax-ns#"
  xmlns:rdfs="http://www.w3.org/2000/01/rdf-schema#"
  xmlns:owl="http://www.w3.org/2002/07/owl#"
  xmlns:xsd="http://www.w3.org/2001/XMLSchema#"
  xml:base="http://example.org/onto/">
  <owl:Class rdf:about="http://example.org/onto/class/google_endpoints_service">
    <rdfs:label>google_endpoints_service</rdfs:label>
    <rdfs:comment>#
#     ***     AUTO GENERATED CODE    ***    Type: Handwritten     ***
#
# ----------------------------------------------------------------------------
#
#     This code is generated by Magic Modules using the following:
#
#     Source file: https://github.com/GoogleCloudPlatform/magic-modules/tree/main/mmv1/third_party/terraform/website/docs/r/endpoints_service.html.markdown
#
#     DO NOT EDIT this file directly. Any changes made to this file will be
#     overwritten during the next generation cycle.
#
# ----------------------------------------------------------------------------
subcategory: "Cloud Endpoints"
description: |-
  Creates and rolls out a Google Endpoints service.
---</rdfs:comment>
  </owl:Class>
  <owl:DatatypeProperty rdf:about="http://example.org/onto/prop/google_endpoints_service_apis">
    <rdfs:label>apis</rdfs:label>
    <rdfs:comment>A list of API objects.</rdfs:comment>
    <rdfs:domain rdf:resource="http://example.org/onto/class/google_endpoints_service"/>
    <rdfs:range rdf:resource="http://www.w3.org/2001/XMLSchema#string"/>
  </owl:DatatypeProperty>
  <owl:DatatypeProperty rdf:about="http://example.org/onto/prop/google_endpoints_service_config_id">
    <rdfs:label>config_id</rdfs:label>
    <rdfs:comment>The autogenerated ID for the configuration that is rolled out as part of the creation of this resource. Must be provided to compute engine instances as a tag.</rdfs:comment>
    <rdfs:domain rdf:resource="http://example.org/onto/class/google_endpoints_service"/>
    <rdfs:range rdf:resource="http://www.w3.org/2001/XMLSchema#string"/>
  </owl:DatatypeProperty>
  <owl:DatatypeProperty rdf:about="http://example.org/onto/prop/google_endpoints_service_dns_address">
    <rdfs:label>dns_address</rdfs:label>
    <rdfs:comment>The address at which the service can be found - usually the same as the service name.</rdfs:comment>
    <rdfs:domain rdf:resource="http://example.org/onto/class/google_endpoints_service"/>
    <rdfs:range rdf:resource="http://www.w3.org/2001/XMLSchema#string"/>
  </owl:DatatypeProperty>
  <owl:DatatypeProperty rdf:about="http://example.org/onto/prop/google_endpoints_service_endpoints">
    <rdfs:label>endpoints</rdfs:label>
    <rdfs:comment>A list of Endpoint objects.</rdfs:comment>
    <rdfs:domain rdf:resource="http://example.org/onto/class/google_endpoints_service"/>
    <rdfs:range rdf:resource="http://www.w3.org/2001/XMLSchema#string"/>
  </owl:DatatypeProperty>
  <owl:DatatypeProperty rdf:about="http://example.org/onto/prop/google_endpoints_service_grpc_config">
    <rdfs:label>grpc_config</rdfs:label>
    <rdfs:comment>The full text of the Service Config YAML file (Example located here). If provided, must also provide protoc_output_base64. open_api config must not be provided.</rdfs:comment>
    <rdfs:domain rdf:resource="http://example.org/onto/class/google_endpoints_service"/>
    <rdfs:range rdf:resource="http://www.w3.org/2001/XMLSchema#string"/>
  </owl:DatatypeProperty>
  <owl:DatatypeProperty rdf:about="http://example.org/onto/prop/google_endpoints_service_id">
    <rdfs:label>id</rdfs:label>
    <rdfs:domain rdf:resource="http://example.org/onto/class/google_endpoints_service"/>
    <rdfs:range rdf:resource="http://www.w3.org/2001/XMLSchema#string"/>
  </owl:DatatypeProperty>
  <owl:DatatypeProperty rdf:about="http://example.org/onto/prop/google_endpoints_service_openapi_config">
    <rdfs:label>openapi_config</rdfs:label>
    <rdfs:comment>The full text of the OpenAPI YAML configuration as described here. Either this, or both of grpc_config and protoc_output_base64 must be specified.</rdfs:comment>
    <rdfs:domain rdf:resource="http://example.org/onto/class/google_endpoints_service"/>
    <rdfs:range rdf:resource="http://www.w3.org/2001/XMLSchema#string"/>
  </owl:DatatypeProperty>
  <owl:DatatypeProperty rdf:about="http://example.org/onto/prop/google_endpoints_service_project">
    <rdfs:label>project</rdfs:label>
    <rdfs:comment>The project ID that the service belongs to. If not provided, provider project is used.</rdfs:comment>
    <rdfs:domain rdf:resource="http://example.org/onto/class/google_endpoints_service"/>
    <rdfs:range rdf:resource="http://www.w3.org/2001/XMLSchema#string"/>
  </owl:DatatypeProperty>
  <owl:DatatypeProperty rdf:about="http://example.org/onto/prop/google_endpoints_service_protoc_output_base64">
    <rdfs:label>protoc_output_base64</rdfs:label>
    <rdfs:comment>The full contents of the Service Descriptor File generated by protoc. This should be a compiled .pb file, base64-encoded.</rdfs:comment>
    <rdfs:domain rdf:resource="http://example.org/onto/class/google_endpoints_service"/>
    <rdfs:range rdf:resource="http://www.w3.org/2001/XMLSchema#string"/>
  </owl:DatatypeProperty>
  <owl:DatatypeProperty rdf:about="http://example.org/onto/prop/google_endpoints_service_service_name">
    <rdfs:label>service_name</rdfs:label>
    <rdfs:comment>The name of the service. Usually of the form $apiname.endpoints.$projectid.cloud.goog.</rdfs:comment>
    <rdfs:domain rdf:resource="http://example.org/onto/class/google_endpoints_service"/>
    <rdfs:range rdf:resource="http://www.w3.org/2001/XMLSchema#string"/>
  </owl:DatatypeProperty>
  <owl:DatatypeProperty rdf:about="http://example.org/onto/prop/google_endpoints_service_create">
    <rdfs:label>create</rdfs:label>
    <rdfs:domain rdf:resource="http://example.org/onto/class/google_endpoints_service"/>
    <rdfs:range rdf:resource="http://www.w3.org/2001/XMLSchema#string"/>
  </owl:DatatypeProperty>
  <owl:DatatypeProperty rdf:about="http://example.org/onto/prop/google_endpoints_service_delete">
    <rdfs:label>delete</rdfs:label>
    <rdfs:domain rdf:resource="http://example.org/onto/class/google_endpoints_service"/>
    <rdfs:range rdf:resource="http://www.w3.org/2001/XMLSchema#string"/>
  </owl:DatatypeProperty>
  <owl:DatatypeProperty rdf:about="http://example.org/onto/prop/google_endpoints_service_update">
    <rdfs:label>update</rdfs:label>
    <rdfs:domain rdf:resource="http://example.org/onto/class/google_endpoints_service"/>
    <rdfs:range rdf:resource="http://www.w3.org/2001/XMLSchema#string"/>
  </owl:DatatypeProperty>
</rdf:RDF>
