<?xml version="1.0" encoding="UTF-8"?>
<rdf:RDF
  xmlns:rdf="http://www.w3.org/1999/02/22-rdf-syntax-ns#"
  xmlns:rdfs="http://www.w3.org/2000/01/rdf-schema#"
  xmlns:owl="http://www.w3.org/2002/07/owl#"
  xmlns:xsd="http://www.w3.org/2001/XMLSchema#"
  xml:base="http://example.org/onto/">
  <owl:Class rdf:about="http://example.org/onto/class/google_data_loss_prevention_job_trigger">
    <rdfs:label>google_data_loss_prevention_job_trigger</rdfs:label>
    <rdfs:comment>#
#     ***     AUTO GENERATED CODE    ***    Type: MMv1     ***
#
# ----------------------------------------------------------------------------
#
#     This code is generated by Magic Modules using the following:
#
#     Configuration: https:#github.com/GoogleCloudPlatform/magic-modules/tree/main/mmv1/products/dlp/JobTrigger.yaml
#     Template:      https:#github.com/GoogleCloudPlatform/magic-modules/tree/main/mmv1/templates/terraform/resource.html.markdown.tmpl
#
#     DO NOT EDIT this file directly. Any changes made to this file will be
#     overwritten during the next generation cycle.
#
# ----------------------------------------------------------------------------
subcategory: "Data Loss Prevention"
description: |-
  A job trigger configuration.
---</rdfs:comment>
  </owl:Class>
  <owl:DatatypeProperty rdf:about="http://example.org/onto/prop/google_data_loss_prevention_job_trigger_create_time">
    <rdfs:label>create_time</rdfs:label>
    <rdfs:comment>The creation timestamp of an inspectTemplate. Set by the server.</rdfs:comment>
    <rdfs:domain rdf:resource="http://example.org/onto/class/google_data_loss_prevention_job_trigger"/>
    <rdfs:range rdf:resource="http://www.w3.org/2001/XMLSchema#string"/>
  </owl:DatatypeProperty>
  <owl:DatatypeProperty rdf:about="http://example.org/onto/prop/google_data_loss_prevention_job_trigger_description">
    <rdfs:label>description</rdfs:label>
    <rdfs:comment>A description of the job trigger.</rdfs:comment>
    <rdfs:domain rdf:resource="http://example.org/onto/class/google_data_loss_prevention_job_trigger"/>
    <rdfs:range rdf:resource="http://www.w3.org/2001/XMLSchema#string"/>
  </owl:DatatypeProperty>
  <owl:DatatypeProperty rdf:about="http://example.org/onto/prop/google_data_loss_prevention_job_trigger_display_name">
    <rdfs:label>display_name</rdfs:label>
    <rdfs:comment>User set display name of the job trigger.</rdfs:comment>
    <rdfs:domain rdf:resource="http://example.org/onto/class/google_data_loss_prevention_job_trigger"/>
    <rdfs:range rdf:resource="http://www.w3.org/2001/XMLSchema#string"/>
  </owl:DatatypeProperty>
  <owl:DatatypeProperty rdf:about="http://example.org/onto/prop/google_data_loss_prevention_job_trigger_id">
    <rdfs:label>id</rdfs:label>
    <rdfs:domain rdf:resource="http://example.org/onto/class/google_data_loss_prevention_job_trigger"/>
    <rdfs:range rdf:resource="http://www.w3.org/2001/XMLSchema#string"/>
  </owl:DatatypeProperty>
  <owl:DatatypeProperty rdf:about="http://example.org/onto/prop/google_data_loss_prevention_job_trigger_last_run_time">
    <rdfs:label>last_run_time</rdfs:label>
    <rdfs:comment>The timestamp of the last time this trigger executed.</rdfs:comment>
    <rdfs:domain rdf:resource="http://example.org/onto/class/google_data_loss_prevention_job_trigger"/>
    <rdfs:range rdf:resource="http://www.w3.org/2001/XMLSchema#string"/>
  </owl:DatatypeProperty>
  <owl:DatatypeProperty rdf:about="http://example.org/onto/prop/google_data_loss_prevention_job_trigger_name">
    <rdfs:label>name</rdfs:label>
    <rdfs:comment>The resource name of the job trigger. Set by the server.</rdfs:comment>
    <rdfs:domain rdf:resource="http://example.org/onto/class/google_data_loss_prevention_job_trigger"/>
    <rdfs:range rdf:resource="http://www.w3.org/2001/XMLSchema#string"/>
  </owl:DatatypeProperty>
  <owl:DatatypeProperty rdf:about="http://example.org/onto/prop/google_data_loss_prevention_job_trigger_parent">
    <rdfs:label>parent</rdfs:label>
    <rdfs:comment>The parent of the trigger, either in the format 'projects/{{project}}'
or 'projects/{{project}}/locations/{{location}}'</rdfs:comment>
    <rdfs:domain rdf:resource="http://example.org/onto/class/google_data_loss_prevention_job_trigger"/>
    <rdfs:range rdf:resource="http://www.w3.org/2001/XMLSchema#string"/>
  </owl:DatatypeProperty>
  <owl:DatatypeProperty rdf:about="http://example.org/onto/prop/google_data_loss_prevention_job_trigger_status">
    <rdfs:label>status</rdfs:label>
    <rdfs:comment>Whether the trigger is currently active. Default value: "HEALTHY" Possible values: ["PAUSED", "HEALTHY", "CANCELLED"]</rdfs:comment>
    <rdfs:domain rdf:resource="http://example.org/onto/class/google_data_loss_prevention_job_trigger"/>
    <rdfs:range rdf:resource="http://www.w3.org/2001/XMLSchema#string"/>
  </owl:DatatypeProperty>
  <owl:DatatypeProperty rdf:about="http://example.org/onto/prop/google_data_loss_prevention_job_trigger_trigger_id">
    <rdfs:label>trigger_id</rdfs:label>
    <rdfs:comment>The trigger id can contain uppercase and lowercase letters, numbers, and hyphens;
that is, it must match the regular expression: [a-zA-Z\d-_]+.
The maximum length is 100 characters. Can be empty to allow the system to generate one.</rdfs:comment>
    <rdfs:domain rdf:resource="http://example.org/onto/class/google_data_loss_prevention_job_trigger"/>
    <rdfs:range rdf:resource="http://www.w3.org/2001/XMLSchema#string"/>
  </owl:DatatypeProperty>
  <owl:DatatypeProperty rdf:about="http://example.org/onto/prop/google_data_loss_prevention_job_trigger_update_time">
    <rdfs:label>update_time</rdfs:label>
    <rdfs:comment>The last update timestamp of an inspectTemplate. Set by the server.</rdfs:comment>
    <rdfs:domain rdf:resource="http://example.org/onto/class/google_data_loss_prevention_job_trigger"/>
    <rdfs:range rdf:resource="http://www.w3.org/2001/XMLSchema#string"/>
  </owl:DatatypeProperty>
  <owl:DatatypeProperty rdf:about="http://example.org/onto/prop/google_data_loss_prevention_job_trigger_inspect_template_name">
    <rdfs:label>inspect_template_name</rdfs:label>
    <rdfs:comment>The name of the template to run when this job is triggered.</rdfs:comment>
    <rdfs:domain rdf:resource="http://example.org/onto/class/google_data_loss_prevention_job_trigger"/>
    <rdfs:range rdf:resource="http://www.w3.org/2001/XMLSchema#string"/>
  </owl:DatatypeProperty>
  <owl:DatatypeProperty rdf:about="http://example.org/onto/prop/google_data_loss_prevention_job_trigger_cloud_storage_output">
    <rdfs:label>cloud_storage_output</rdfs:label>
    <rdfs:comment>User settable Cloud Storage bucket and folders to store de-identified files.

This field must be set for cloud storage deidentification.

The output Cloud Storage bucket must be different from the input bucket.

De-identified files will overwrite files in the output path.

Form of: gs://bucket/folder/ or gs://bucket</rdfs:comment>
    <rdfs:domain rdf:resource="http://example.org/onto/class/google_data_loss_prevention_job_trigger"/>
    <rdfs:range rdf:resource="http://www.w3.org/2001/XMLSchema#string"/>
  </owl:DatatypeProperty>
  <owl:DatatypeProperty rdf:about="http://example.org/onto/prop/google_data_loss_prevention_job_trigger_file_types_to_transform">
    <rdfs:label>file_types_to_transform</rdfs:label>
    <rdfs:comment>List of user-specified file type groups to transform. If specified, only the files with these filetypes will be transformed.

If empty, all supported files will be transformed. Supported types may be automatically added over time.

If a file type is set in this field that isn't supported by the Deidentify action then the job will fail and will not be successfully created/started. Possible values: ["IMAGE", "TEXT_FILE", "CSV", "TSV"]</rdfs:comment>
    <rdfs:domain rdf:resource="http://example.org/onto/class/google_data_loss_prevention_job_trigger"/>
    <rdfs:range rdf:resource="http://www.w3.org/2001/XMLSchema#string"/>
  </owl:DatatypeProperty>
  <owl:DatatypeProperty rdf:about="http://example.org/onto/prop/google_data_loss_prevention_job_trigger_deidentify_template">
    <rdfs:label>deidentify_template</rdfs:label>
    <rdfs:comment>If this template is specified, it will serve as the default de-identify template.</rdfs:comment>
    <rdfs:domain rdf:resource="http://example.org/onto/class/google_data_loss_prevention_job_trigger"/>
    <rdfs:range rdf:resource="http://www.w3.org/2001/XMLSchema#string"/>
  </owl:DatatypeProperty>
  <owl:DatatypeProperty rdf:about="http://example.org/onto/prop/google_data_loss_prevention_job_trigger_image_redact_template">
    <rdfs:label>image_redact_template</rdfs:label>
    <rdfs:comment>If this template is specified, it will serve as the de-identify template for images.</rdfs:comment>
    <rdfs:domain rdf:resource="http://example.org/onto/class/google_data_loss_prevention_job_trigger"/>
    <rdfs:range rdf:resource="http://www.w3.org/2001/XMLSchema#string"/>
  </owl:DatatypeProperty>
  <owl:DatatypeProperty rdf:about="http://example.org/onto/prop/google_data_loss_prevention_job_trigger_structured_deidentify_template">
    <rdfs:label>structured_deidentify_template</rdfs:label>
    <rdfs:comment>If this template is specified, it will serve as the de-identify template for structured content such as delimited files and tables.</rdfs:comment>
    <rdfs:domain rdf:resource="http://example.org/onto/class/google_data_loss_prevention_job_trigger"/>
    <rdfs:range rdf:resource="http://www.w3.org/2001/XMLSchema#string"/>
  </owl:DatatypeProperty>
  <owl:DatatypeProperty rdf:about="http://example.org/onto/prop/google_data_loss_prevention_job_trigger_dataset_id">
    <rdfs:label>dataset_id</rdfs:label>
    <rdfs:comment>The ID of the dataset containing this table.</rdfs:comment>
    <rdfs:domain rdf:resource="http://example.org/onto/class/google_data_loss_prevention_job_trigger"/>
    <rdfs:range rdf:resource="http://www.w3.org/2001/XMLSchema#string"/>
  </owl:DatatypeProperty>
  <owl:DatatypeProperty rdf:about="http://example.org/onto/prop/google_data_loss_prevention_job_trigger_project_id">
    <rdfs:label>project_id</rdfs:label>
    <rdfs:comment>The ID of the project containing this table.</rdfs:comment>
    <rdfs:domain rdf:resource="http://example.org/onto/class/google_data_loss_prevention_job_trigger"/>
    <rdfs:range rdf:resource="http://www.w3.org/2001/XMLSchema#string"/>
  </owl:DatatypeProperty>
  <owl:DatatypeProperty rdf:about="http://example.org/onto/prop/google_data_loss_prevention_job_trigger_table_id">
    <rdfs:label>table_id</rdfs:label>
    <rdfs:comment>The ID of the table. The ID must contain only letters (a-z,
A-Z), numbers (0-9), or underscores (_). The maximum length
is 1,024 characters.</rdfs:comment>
    <rdfs:domain rdf:resource="http://example.org/onto/class/google_data_loss_prevention_job_trigger"/>
    <rdfs:range rdf:resource="http://www.w3.org/2001/XMLSchema#string"/>
  </owl:DatatypeProperty>
  <owl:DatatypeProperty rdf:about="http://example.org/onto/prop/google_data_loss_prevention_job_trigger_topic">
    <rdfs:label>topic</rdfs:label>
    <rdfs:comment>Cloud Pub/Sub topic to send notifications to.</rdfs:comment>
    <rdfs:domain rdf:resource="http://example.org/onto/class/google_data_loss_prevention_job_trigger"/>
    <rdfs:range rdf:resource="http://www.w3.org/2001/XMLSchema#string"/>
  </owl:DatatypeProperty>
  <owl:DatatypeProperty rdf:about="http://example.org/onto/prop/google_data_loss_prevention_job_trigger_output_schema">
    <rdfs:label>output_schema</rdfs:label>
    <rdfs:comment>Schema used for writing the findings for Inspect jobs. This field is only used for
Inspect and must be unspecified for Risk jobs. Columns are derived from the Finding
object. If appending to an existing table, any columns from the predefined schema
that are missing will be added. No columns in the existing table will be deleted.

If unspecified, then all available columns will be used for a new table or an (existing)
table with no schema, and no changes will be made to an existing table that has a schema.
Only for use with external storage. Possible values: ["BASIC_COLUMNS", "GCS_COLUMNS", "DATASTORE_COLUMNS", "BIG_QUERY_COLUMNS", "ALL_COLUMNS"]</rdfs:comment>
    <rdfs:domain rdf:resource="http://example.org/onto/class/google_data_loss_prevention_job_trigger"/>
    <rdfs:range rdf:resource="http://www.w3.org/2001/XMLSchema#string"/>
  </owl:DatatypeProperty>
  <owl:DatatypeProperty rdf:about="http://example.org/onto/prop/google_data_loss_prevention_job_trigger_path">
    <rdfs:label>path</rdfs:label>
    <rdfs:comment>A URL representing a file or path (no wildcards) in Cloud Storage.
Example: 'gs://[BUCKET_NAME]/dictionary.txt'</rdfs:comment>
    <rdfs:domain rdf:resource="http://example.org/onto/class/google_data_loss_prevention_job_trigger"/>
    <rdfs:range rdf:resource="http://www.w3.org/2001/XMLSchema#string"/>
  </owl:DatatypeProperty>
  <owl:DatatypeProperty rdf:about="http://example.org/onto/prop/google_data_loss_prevention_job_trigger_dataset_id">
    <rdfs:label>dataset_id</rdfs:label>
    <rdfs:comment>Dataset ID of the table.</rdfs:comment>
    <rdfs:domain rdf:resource="http://example.org/onto/class/google_data_loss_prevention_job_trigger"/>
    <rdfs:range rdf:resource="http://www.w3.org/2001/XMLSchema#string"/>
  </owl:DatatypeProperty>
  <owl:DatatypeProperty rdf:about="http://example.org/onto/prop/google_data_loss_prevention_job_trigger_project_id">
    <rdfs:label>project_id</rdfs:label>
    <rdfs:comment>The Google Cloud Platform project ID of the project containing the table.</rdfs:comment>
    <rdfs:domain rdf:resource="http://example.org/onto/class/google_data_loss_prevention_job_trigger"/>
    <rdfs:range rdf:resource="http://www.w3.org/2001/XMLSchema#string"/>
  </owl:DatatypeProperty>
  <owl:DatatypeProperty rdf:about="http://example.org/onto/prop/google_data_loss_prevention_job_trigger_table_id">
    <rdfs:label>table_id</rdfs:label>
    <rdfs:comment>Name of the table. If is not set a new one will be generated for you with the following format:
'dlp_googleapis_yyyy_mm_dd_[dlp_job_id]'. Pacific timezone will be used for generating the date details.</rdfs:comment>
    <rdfs:domain rdf:resource="http://example.org/onto/class/google_data_loss_prevention_job_trigger"/>
    <rdfs:range rdf:resource="http://www.w3.org/2001/XMLSchema#string"/>
  </owl:DatatypeProperty>
  <owl:DatatypeProperty rdf:about="http://example.org/onto/prop/google_data_loss_prevention_job_trigger_exclude_info_types">
    <rdfs:label>exclude_info_types</rdfs:label>
    <rdfs:comment>When true, excludes type information of the findings.</rdfs:comment>
    <rdfs:domain rdf:resource="http://example.org/onto/class/google_data_loss_prevention_job_trigger"/>
    <rdfs:range rdf:resource="http://www.w3.org/2001/XMLSchema#string"/>
  </owl:DatatypeProperty>
  <owl:DatatypeProperty rdf:about="http://example.org/onto/prop/google_data_loss_prevention_job_trigger_include_quote">
    <rdfs:label>include_quote</rdfs:label>
    <rdfs:comment>When true, a contextual quote from the data that triggered a finding is included in the response.</rdfs:comment>
    <rdfs:domain rdf:resource="http://example.org/onto/class/google_data_loss_prevention_job_trigger"/>
    <rdfs:range rdf:resource="http://www.w3.org/2001/XMLSchema#string"/>
  </owl:DatatypeProperty>
  <owl:DatatypeProperty rdf:about="http://example.org/onto/prop/google_data_loss_prevention_job_trigger_min_likelihood">
    <rdfs:label>min_likelihood</rdfs:label>
    <rdfs:comment>Only returns findings equal or above this threshold. See https://cloud.google.com/dlp/docs/likelihood for more info Default value: "POSSIBLE" Possible values: ["VERY_UNLIKELY", "UNLIKELY", "POSSIBLE", "LIKELY", "VERY_LIKELY"]</rdfs:comment>
    <rdfs:domain rdf:resource="http://example.org/onto/class/google_data_loss_prevention_job_trigger"/>
    <rdfs:range rdf:resource="http://www.w3.org/2001/XMLSchema#string"/>
  </owl:DatatypeProperty>
  <owl:DatatypeProperty rdf:about="http://example.org/onto/prop/google_data_loss_prevention_job_trigger_exclusion_type">
    <rdfs:label>exclusion_type</rdfs:label>
    <rdfs:comment>If set to EXCLUSION_TYPE_EXCLUDE this infoType will not cause a finding to be returned. It still can be used for rules matching. Possible values: ["EXCLUSION_TYPE_EXCLUDE"]</rdfs:comment>
    <rdfs:domain rdf:resource="http://example.org/onto/class/google_data_loss_prevention_job_trigger"/>
    <rdfs:range rdf:resource="http://www.w3.org/2001/XMLSchema#string"/>
  </owl:DatatypeProperty>
  <owl:DatatypeProperty rdf:about="http://example.org/onto/prop/google_data_loss_prevention_job_trigger_likelihood">
    <rdfs:label>likelihood</rdfs:label>
    <rdfs:comment>Likelihood to return for this CustomInfoType. This base value can be altered by a detection rule if the finding meets the criteria
specified by the rule. Default value: "VERY_LIKELY" Possible values: ["VERY_UNLIKELY", "UNLIKELY", "POSSIBLE", "LIKELY", "VERY_LIKELY"]</rdfs:comment>
    <rdfs:domain rdf:resource="http://example.org/onto/class/google_data_loss_prevention_job_trigger"/>
    <rdfs:range rdf:resource="http://www.w3.org/2001/XMLSchema#string"/>
  </owl:DatatypeProperty>
  <owl:DatatypeProperty rdf:about="http://example.org/onto/prop/google_data_loss_prevention_job_trigger_path">
    <rdfs:label>path</rdfs:label>
    <rdfs:comment>A url representing a file or path (no wildcards) in Cloud Storage. Example: 'gs://[BUCKET_NAME]/dictionary.txt'</rdfs:comment>
    <rdfs:domain rdf:resource="http://example.org/onto/class/google_data_loss_prevention_job_trigger"/>
    <rdfs:range rdf:resource="http://www.w3.org/2001/XMLSchema#string"/>
  </owl:DatatypeProperty>
  <owl:DatatypeProperty rdf:about="http://example.org/onto/prop/google_data_loss_prevention_job_trigger_words">
    <rdfs:label>words</rdfs:label>
    <rdfs:comment>Words or phrases defining the dictionary. The dictionary must contain at least one
phrase and every phrase must contain at least 2 characters that are letters or digits.</rdfs:comment>
    <rdfs:domain rdf:resource="http://example.org/onto/class/google_data_loss_prevention_job_trigger"/>
    <rdfs:range rdf:resource="http://www.w3.org/2001/XMLSchema#string"/>
  </owl:DatatypeProperty>
  <owl:DatatypeProperty rdf:about="http://example.org/onto/prop/google_data_loss_prevention_job_trigger_name">
    <rdfs:label>name</rdfs:label>
    <rdfs:comment>Name of the information type. Either a name of your choosing when creating a CustomInfoType, or one of the names
listed at https://cloud.google.com/dlp/docs/infotypes-reference when specifying a built-in type.</rdfs:comment>
    <rdfs:domain rdf:resource="http://example.org/onto/class/google_data_loss_prevention_job_trigger"/>
    <rdfs:range rdf:resource="http://www.w3.org/2001/XMLSchema#string"/>
  </owl:DatatypeProperty>
  <owl:DatatypeProperty rdf:about="http://example.org/onto/prop/google_data_loss_prevention_job_trigger_version">
    <rdfs:label>version</rdfs:label>
    <rdfs:comment>Version of the information type to use. By default, the version is set to stable.</rdfs:comment>
    <rdfs:domain rdf:resource="http://example.org/onto/class/google_data_loss_prevention_job_trigger"/>
    <rdfs:range rdf:resource="http://www.w3.org/2001/XMLSchema#string"/>
  </owl:DatatypeProperty>
  <owl:DatatypeProperty rdf:about="http://example.org/onto/prop/google_data_loss_prevention_job_trigger_score">
    <rdfs:label>score</rdfs:label>
    <rdfs:comment>The sensitivity score applied to the resource. Possible values: ["SENSITIVITY_LOW", "SENSITIVITY_MODERATE", "SENSITIVITY_HIGH"]</rdfs:comment>
    <rdfs:domain rdf:resource="http://example.org/onto/class/google_data_loss_prevention_job_trigger"/>
    <rdfs:range rdf:resource="http://www.w3.org/2001/XMLSchema#string"/>
  </owl:DatatypeProperty>
  <owl:DatatypeProperty rdf:about="http://example.org/onto/prop/google_data_loss_prevention_job_trigger_group_indexes">
    <rdfs:label>group_indexes</rdfs:label>
    <rdfs:comment>The index of the submatch to extract as findings. When not specified, the entire match is returned. No more than 3 may be included.</rdfs:comment>
    <rdfs:domain rdf:resource="http://example.org/onto/class/google_data_loss_prevention_job_trigger"/>
    <rdfs:range rdf:resource="http://www.w3.org/2001/XMLSchema#string"/>
  </owl:DatatypeProperty>
  <owl:DatatypeProperty rdf:about="http://example.org/onto/prop/google_data_loss_prevention_job_trigger_pattern">
    <rdfs:label>pattern</rdfs:label>
    <rdfs:comment>Pattern defining the regular expression.
Its syntax (https://github.com/google/re2/wiki/Syntax) can be found under the google/re2 repository on GitHub.</rdfs:comment>
    <rdfs:domain rdf:resource="http://example.org/onto/class/google_data_loss_prevention_job_trigger"/>
    <rdfs:range rdf:resource="http://www.w3.org/2001/XMLSchema#string"/>
  </owl:DatatypeProperty>
  <owl:DatatypeProperty rdf:about="http://example.org/onto/prop/google_data_loss_prevention_job_trigger_score">
    <rdfs:label>score</rdfs:label>
    <rdfs:comment>The sensitivity score applied to the resource. Possible values: ["SENSITIVITY_LOW", "SENSITIVITY_MODERATE", "SENSITIVITY_HIGH"]</rdfs:comment>
    <rdfs:domain rdf:resource="http://example.org/onto/class/google_data_loss_prevention_job_trigger"/>
    <rdfs:range rdf:resource="http://www.w3.org/2001/XMLSchema#string"/>
  </owl:DatatypeProperty>
  <owl:DatatypeProperty rdf:about="http://example.org/onto/prop/google_data_loss_prevention_job_trigger_create_time">
    <rdfs:label>create_time</rdfs:label>
    <rdfs:comment>The creation timestamp of an inspectTemplate. Set by the server.</rdfs:comment>
    <rdfs:domain rdf:resource="http://example.org/onto/class/google_data_loss_prevention_job_trigger"/>
    <rdfs:range rdf:resource="http://www.w3.org/2001/XMLSchema#string"/>
  </owl:DatatypeProperty>
  <owl:DatatypeProperty rdf:about="http://example.org/onto/prop/google_data_loss_prevention_job_trigger_name">
    <rdfs:label>name</rdfs:label>
    <rdfs:comment>Resource name of the requested StoredInfoType, for example 'organizations/433245324/storedInfoTypes/432452342'
or 'projects/project-id/storedInfoTypes/432452342'.</rdfs:comment>
    <rdfs:domain rdf:resource="http://example.org/onto/class/google_data_loss_prevention_job_trigger"/>
    <rdfs:range rdf:resource="http://www.w3.org/2001/XMLSchema#string"/>
  </owl:DatatypeProperty>
  <owl:DatatypeProperty rdf:about="http://example.org/onto/prop/google_data_loss_prevention_job_trigger_name">
    <rdfs:label>name</rdfs:label>
    <rdfs:comment>Name of the information type. Either a name of your choosing when creating a CustomInfoType, or one of the names listed
at https://cloud.google.com/dlp/docs/infotypes-reference when specifying a built-in type.</rdfs:comment>
    <rdfs:domain rdf:resource="http://example.org/onto/class/google_data_loss_prevention_job_trigger"/>
    <rdfs:range rdf:resource="http://www.w3.org/2001/XMLSchema#string"/>
  </owl:DatatypeProperty>
  <owl:DatatypeProperty rdf:about="http://example.org/onto/prop/google_data_loss_prevention_job_trigger_version">
    <rdfs:label>version</rdfs:label>
    <rdfs:comment>Version of the information type to use. By default, the version is set to stable</rdfs:comment>
    <rdfs:domain rdf:resource="http://example.org/onto/class/google_data_loss_prevention_job_trigger"/>
    <rdfs:range rdf:resource="http://www.w3.org/2001/XMLSchema#string"/>
  </owl:DatatypeProperty>
  <owl:DatatypeProperty rdf:about="http://example.org/onto/prop/google_data_loss_prevention_job_trigger_score">
    <rdfs:label>score</rdfs:label>
    <rdfs:comment>The sensitivity score applied to the resource. Possible values: ["SENSITIVITY_LOW", "SENSITIVITY_MODERATE", "SENSITIVITY_HIGH"]</rdfs:comment>
    <rdfs:domain rdf:resource="http://example.org/onto/class/google_data_loss_prevention_job_trigger"/>
    <rdfs:range rdf:resource="http://www.w3.org/2001/XMLSchema#string"/>
  </owl:DatatypeProperty>
  <owl:DatatypeProperty rdf:about="http://example.org/onto/prop/google_data_loss_prevention_job_trigger_max_findings_per_item">
    <rdfs:label>max_findings_per_item</rdfs:label>
    <rdfs:comment>Max number of findings that will be returned for each item scanned. The maximum returned is 2000.</rdfs:comment>
    <rdfs:domain rdf:resource="http://example.org/onto/class/google_data_loss_prevention_job_trigger"/>
    <rdfs:range rdf:resource="http://www.w3.org/2001/XMLSchema#string"/>
  </owl:DatatypeProperty>
  <owl:DatatypeProperty rdf:about="http://example.org/onto/prop/google_data_loss_prevention_job_trigger_max_findings_per_request">
    <rdfs:label>max_findings_per_request</rdfs:label>
    <rdfs:comment>Max number of findings that will be returned per request/job. The maximum returned is 2000.</rdfs:comment>
    <rdfs:domain rdf:resource="http://example.org/onto/class/google_data_loss_prevention_job_trigger"/>
    <rdfs:range rdf:resource="http://www.w3.org/2001/XMLSchema#string"/>
  </owl:DatatypeProperty>
  <owl:DatatypeProperty rdf:about="http://example.org/onto/prop/google_data_loss_prevention_job_trigger_max_findings">
    <rdfs:label>max_findings</rdfs:label>
    <rdfs:comment>Max findings limit for the given infoType.</rdfs:comment>
    <rdfs:domain rdf:resource="http://example.org/onto/class/google_data_loss_prevention_job_trigger"/>
    <rdfs:range rdf:resource="http://www.w3.org/2001/XMLSchema#string"/>
  </owl:DatatypeProperty>
  <owl:DatatypeProperty rdf:about="http://example.org/onto/prop/google_data_loss_prevention_job_trigger_name">
    <rdfs:label>name</rdfs:label>
    <rdfs:comment>Name of the information type. Either a name of your choosing when creating a CustomInfoType, or one of the names listed
at https://cloud.google.com/dlp/docs/infotypes-reference when specifying a built-in type.</rdfs:comment>
    <rdfs:domain rdf:resource="http://example.org/onto/class/google_data_loss_prevention_job_trigger"/>
    <rdfs:range rdf:resource="http://www.w3.org/2001/XMLSchema#string"/>
  </owl:DatatypeProperty>
  <owl:DatatypeProperty rdf:about="http://example.org/onto/prop/google_data_loss_prevention_job_trigger_version">
    <rdfs:label>version</rdfs:label>
    <rdfs:comment>Version of the information type to use. By default, the version is set to stable</rdfs:comment>
    <rdfs:domain rdf:resource="http://example.org/onto/class/google_data_loss_prevention_job_trigger"/>
    <rdfs:range rdf:resource="http://www.w3.org/2001/XMLSchema#string"/>
  </owl:DatatypeProperty>
  <owl:DatatypeProperty rdf:about="http://example.org/onto/prop/google_data_loss_prevention_job_trigger_score">
    <rdfs:label>score</rdfs:label>
    <rdfs:comment>The sensitivity score applied to the resource. Possible values: ["SENSITIVITY_LOW", "SENSITIVITY_MODERATE", "SENSITIVITY_HIGH"]</rdfs:comment>
    <rdfs:domain rdf:resource="http://example.org/onto/class/google_data_loss_prevention_job_trigger"/>
    <rdfs:range rdf:resource="http://www.w3.org/2001/XMLSchema#string"/>
  </owl:DatatypeProperty>
  <owl:DatatypeProperty rdf:about="http://example.org/onto/prop/google_data_loss_prevention_job_trigger_name">
    <rdfs:label>name</rdfs:label>
    <rdfs:comment>Name of the information type. Either a name of your choosing when creating a CustomInfoType, or one of the names listed
at https://cloud.google.com/dlp/docs/infotypes-reference when specifying a built-in type.</rdfs:comment>
    <rdfs:domain rdf:resource="http://example.org/onto/class/google_data_loss_prevention_job_trigger"/>
    <rdfs:range rdf:resource="http://www.w3.org/2001/XMLSchema#string"/>
  </owl:DatatypeProperty>
  <owl:DatatypeProperty rdf:about="http://example.org/onto/prop/google_data_loss_prevention_job_trigger_version">
    <rdfs:label>version</rdfs:label>
    <rdfs:comment>Version of the information type to use. By default, the version is set to stable.</rdfs:comment>
    <rdfs:domain rdf:resource="http://example.org/onto/class/google_data_loss_prevention_job_trigger"/>
    <rdfs:range rdf:resource="http://www.w3.org/2001/XMLSchema#string"/>
  </owl:DatatypeProperty>
  <owl:DatatypeProperty rdf:about="http://example.org/onto/prop/google_data_loss_prevention_job_trigger_score">
    <rdfs:label>score</rdfs:label>
    <rdfs:comment>The sensitivity score applied to the resource. Possible values: ["SENSITIVITY_LOW", "SENSITIVITY_MODERATE", "SENSITIVITY_HIGH"]</rdfs:comment>
    <rdfs:domain rdf:resource="http://example.org/onto/class/google_data_loss_prevention_job_trigger"/>
    <rdfs:range rdf:resource="http://www.w3.org/2001/XMLSchema#string"/>
  </owl:DatatypeProperty>
  <owl:DatatypeProperty rdf:about="http://example.org/onto/prop/google_data_loss_prevention_job_trigger_matching_type">
    <rdfs:label>matching_type</rdfs:label>
    <rdfs:comment>How the rule is applied. See the documentation for more information: https://cloud.google.com/dlp/docs/reference/rest/v2/InspectConfig#MatchingType Possible values: ["MATCHING_TYPE_FULL_MATCH", "MATCHING_TYPE_PARTIAL_MATCH", "MATCHING_TYPE_INVERSE_MATCH"]</rdfs:comment>
    <rdfs:domain rdf:resource="http://example.org/onto/class/google_data_loss_prevention_job_trigger"/>
    <rdfs:range rdf:resource="http://www.w3.org/2001/XMLSchema#string"/>
  </owl:DatatypeProperty>
  <owl:DatatypeProperty rdf:about="http://example.org/onto/prop/google_data_loss_prevention_job_trigger_path">
    <rdfs:label>path</rdfs:label>
    <rdfs:comment>A url representing a file or path (no wildcards) in Cloud Storage. Example: 'gs://[BUCKET_NAME]/dictionary.txt'</rdfs:comment>
    <rdfs:domain rdf:resource="http://example.org/onto/class/google_data_loss_prevention_job_trigger"/>
    <rdfs:range rdf:resource="http://www.w3.org/2001/XMLSchema#string"/>
  </owl:DatatypeProperty>
  <owl:DatatypeProperty rdf:about="http://example.org/onto/prop/google_data_loss_prevention_job_trigger_words">
    <rdfs:label>words</rdfs:label>
    <rdfs:comment>Words or phrases defining the dictionary. The dictionary must contain at least one
phrase and every phrase must contain at least 2 characters that are letters or digits.</rdfs:comment>
    <rdfs:domain rdf:resource="http://example.org/onto/class/google_data_loss_prevention_job_trigger"/>
    <rdfs:range rdf:resource="http://www.w3.org/2001/XMLSchema#string"/>
  </owl:DatatypeProperty>
  <owl:DatatypeProperty rdf:about="http://example.org/onto/prop/google_data_loss_prevention_job_trigger_group_indexes">
    <rdfs:label>group_indexes</rdfs:label>
    <rdfs:comment>The index of the submatch to extract as findings. When not specified,
the entire match is returned. No more than 3 may be included.</rdfs:comment>
    <rdfs:domain rdf:resource="http://example.org/onto/class/google_data_loss_prevention_job_trigger"/>
    <rdfs:range rdf:resource="http://www.w3.org/2001/XMLSchema#string"/>
  </owl:DatatypeProperty>
  <owl:DatatypeProperty rdf:about="http://example.org/onto/prop/google_data_loss_prevention_job_trigger_pattern">
    <rdfs:label>pattern</rdfs:label>
    <rdfs:comment>Pattern defining the regular expression. Its syntax
(https://github.com/google/re2/wiki/Syntax) can be found under the google/re2 repository on GitHub.</rdfs:comment>
    <rdfs:domain rdf:resource="http://example.org/onto/class/google_data_loss_prevention_job_trigger"/>
    <rdfs:range rdf:resource="http://www.w3.org/2001/XMLSchema#string"/>
  </owl:DatatypeProperty>
  <owl:DatatypeProperty rdf:about="http://example.org/onto/prop/google_data_loss_prevention_job_trigger_window_after">
    <rdfs:label>window_after</rdfs:label>
    <rdfs:comment>Number of characters after the finding to consider. Either this or window_before must be specified</rdfs:comment>
    <rdfs:domain rdf:resource="http://example.org/onto/class/google_data_loss_prevention_job_trigger"/>
    <rdfs:range rdf:resource="http://www.w3.org/2001/XMLSchema#string"/>
  </owl:DatatypeProperty>
  <owl:DatatypeProperty rdf:about="http://example.org/onto/prop/google_data_loss_prevention_job_trigger_window_before">
    <rdfs:label>window_before</rdfs:label>
    <rdfs:comment>Number of characters before the finding to consider. Either this or window_after must be specified</rdfs:comment>
    <rdfs:domain rdf:resource="http://example.org/onto/class/google_data_loss_prevention_job_trigger"/>
    <rdfs:range rdf:resource="http://www.w3.org/2001/XMLSchema#string"/>
  </owl:DatatypeProperty>
  <owl:DatatypeProperty rdf:about="http://example.org/onto/prop/google_data_loss_prevention_job_trigger_name">
    <rdfs:label>name</rdfs:label>
    <rdfs:comment>Name of the information type. Either a name of your choosing when creating a CustomInfoType, or one of the names listed
at https://cloud.google.com/dlp/docs/infotypes-reference when specifying a built-in type.</rdfs:comment>
    <rdfs:domain rdf:resource="http://example.org/onto/class/google_data_loss_prevention_job_trigger"/>
    <rdfs:range rdf:resource="http://www.w3.org/2001/XMLSchema#string"/>
  </owl:DatatypeProperty>
  <owl:DatatypeProperty rdf:about="http://example.org/onto/prop/google_data_loss_prevention_job_trigger_version">
    <rdfs:label>version</rdfs:label>
    <rdfs:comment>Version of the information type to use. By default, the version is set to stable.</rdfs:comment>
    <rdfs:domain rdf:resource="http://example.org/onto/class/google_data_loss_prevention_job_trigger"/>
    <rdfs:range rdf:resource="http://www.w3.org/2001/XMLSchema#string"/>
  </owl:DatatypeProperty>
  <owl:DatatypeProperty rdf:about="http://example.org/onto/prop/google_data_loss_prevention_job_trigger_score">
    <rdfs:label>score</rdfs:label>
    <rdfs:comment>The sensitivity score applied to the resource. Possible values: ["SENSITIVITY_LOW", "SENSITIVITY_MODERATE", "SENSITIVITY_HIGH"]</rdfs:comment>
    <rdfs:domain rdf:resource="http://example.org/onto/class/google_data_loss_prevention_job_trigger"/>
    <rdfs:range rdf:resource="http://www.w3.org/2001/XMLSchema#string"/>
  </owl:DatatypeProperty>
  <owl:DatatypeProperty rdf:about="http://example.org/onto/prop/google_data_loss_prevention_job_trigger_group_indexes">
    <rdfs:label>group_indexes</rdfs:label>
    <rdfs:comment>The index of the submatch to extract as findings. When not specified, the entire match is returned. No more than 3 may be included.</rdfs:comment>
    <rdfs:domain rdf:resource="http://example.org/onto/class/google_data_loss_prevention_job_trigger"/>
    <rdfs:range rdf:resource="http://www.w3.org/2001/XMLSchema#string"/>
  </owl:DatatypeProperty>
  <owl:DatatypeProperty rdf:about="http://example.org/onto/prop/google_data_loss_prevention_job_trigger_pattern">
    <rdfs:label>pattern</rdfs:label>
    <rdfs:comment>Pattern defining the regular expression.
Its syntax (https://github.com/google/re2/wiki/Syntax) can be found under the google/re2 repository on GitHub.</rdfs:comment>
    <rdfs:domain rdf:resource="http://example.org/onto/class/google_data_loss_prevention_job_trigger"/>
    <rdfs:range rdf:resource="http://www.w3.org/2001/XMLSchema#string"/>
  </owl:DatatypeProperty>
  <owl:DatatypeProperty rdf:about="http://example.org/onto/prop/google_data_loss_prevention_job_trigger_group_indexes">
    <rdfs:label>group_indexes</rdfs:label>
    <rdfs:comment>The index of the submatch to extract as findings. When not specified,
the entire match is returned. No more than 3 may be included.</rdfs:comment>
    <rdfs:domain rdf:resource="http://example.org/onto/class/google_data_loss_prevention_job_trigger"/>
    <rdfs:range rdf:resource="http://www.w3.org/2001/XMLSchema#string"/>
  </owl:DatatypeProperty>
  <owl:DatatypeProperty rdf:about="http://example.org/onto/prop/google_data_loss_prevention_job_trigger_pattern">
    <rdfs:label>pattern</rdfs:label>
    <rdfs:comment>Pattern defining the regular expression. Its syntax
(https://github.com/google/re2/wiki/Syntax) can be found under the google/re2 repository on GitHub.</rdfs:comment>
    <rdfs:domain rdf:resource="http://example.org/onto/class/google_data_loss_prevention_job_trigger"/>
    <rdfs:range rdf:resource="http://www.w3.org/2001/XMLSchema#string"/>
  </owl:DatatypeProperty>
  <owl:DatatypeProperty rdf:about="http://example.org/onto/prop/google_data_loss_prevention_job_trigger_fixed_likelihood">
    <rdfs:label>fixed_likelihood</rdfs:label>
    <rdfs:comment>Set the likelihood of a finding to a fixed value. Either this or relative_likelihood can be set. Possible values: ["VERY_UNLIKELY", "UNLIKELY", "POSSIBLE", "LIKELY", "VERY_LIKELY"]</rdfs:comment>
    <rdfs:domain rdf:resource="http://example.org/onto/class/google_data_loss_prevention_job_trigger"/>
    <rdfs:range rdf:resource="http://www.w3.org/2001/XMLSchema#string"/>
  </owl:DatatypeProperty>
  <owl:DatatypeProperty rdf:about="http://example.org/onto/prop/google_data_loss_prevention_job_trigger_relative_likelihood">
    <rdfs:label>relative_likelihood</rdfs:label>
    <rdfs:comment>Increase or decrease the likelihood by the specified number of levels. For example,
if a finding would be POSSIBLE without the detection rule and relativeLikelihood is 1,
then it is upgraded to LIKELY, while a value of -1 would downgrade it to UNLIKELY.
Likelihood may never drop below VERY_UNLIKELY or exceed VERY_LIKELY, so applying an
adjustment of 1 followed by an adjustment of -1 when base likelihood is VERY_LIKELY
will result in a final likelihood of LIKELY. Either this or fixed_likelihood can be set.</rdfs:comment>
    <rdfs:domain rdf:resource="http://example.org/onto/class/google_data_loss_prevention_job_trigger"/>
    <rdfs:range rdf:resource="http://www.w3.org/2001/XMLSchema#string"/>
  </owl:DatatypeProperty>
  <owl:DatatypeProperty rdf:about="http://example.org/onto/prop/google_data_loss_prevention_job_trigger_window_after">
    <rdfs:label>window_after</rdfs:label>
    <rdfs:comment>Number of characters after the finding to consider. Either this or window_before must be specified</rdfs:comment>
    <rdfs:domain rdf:resource="http://example.org/onto/class/google_data_loss_prevention_job_trigger"/>
    <rdfs:range rdf:resource="http://www.w3.org/2001/XMLSchema#string"/>
  </owl:DatatypeProperty>
  <owl:DatatypeProperty rdf:about="http://example.org/onto/prop/google_data_loss_prevention_job_trigger_window_before">
    <rdfs:label>window_before</rdfs:label>
    <rdfs:comment>Number of characters before the finding to consider. Either this or window_after must be specified</rdfs:comment>
    <rdfs:domain rdf:resource="http://example.org/onto/class/google_data_loss_prevention_job_trigger"/>
    <rdfs:range rdf:resource="http://www.w3.org/2001/XMLSchema#string"/>
  </owl:DatatypeProperty>
  <owl:DatatypeProperty rdf:about="http://example.org/onto/prop/google_data_loss_prevention_job_trigger_rows_limit">
    <rdfs:label>rows_limit</rdfs:label>
    <rdfs:comment>Max number of rows to scan. If the table has more rows than this value, the rest of the rows are omitted.
If not set, or if set to 0, all rows will be scanned. Only one of rowsLimit and rowsLimitPercent can be
specified. Cannot be used in conjunction with TimespanConfig.</rdfs:comment>
    <rdfs:domain rdf:resource="http://example.org/onto/class/google_data_loss_prevention_job_trigger"/>
    <rdfs:range rdf:resource="http://www.w3.org/2001/XMLSchema#string"/>
  </owl:DatatypeProperty>
  <owl:DatatypeProperty rdf:about="http://example.org/onto/prop/google_data_loss_prevention_job_trigger_rows_limit_percent">
    <rdfs:label>rows_limit_percent</rdfs:label>
    <rdfs:comment>Max percentage of rows to scan. The rest are omitted. The number of rows scanned is rounded down.
Must be between 0 and 100, inclusively. Both 0 and 100 means no limit. Defaults to 0. Only one of
rowsLimit and rowsLimitPercent can be specified. Cannot be used in conjunction with TimespanConfig.</rdfs:comment>
    <rdfs:domain rdf:resource="http://example.org/onto/class/google_data_loss_prevention_job_trigger"/>
    <rdfs:range rdf:resource="http://www.w3.org/2001/XMLSchema#string"/>
  </owl:DatatypeProperty>
  <owl:DatatypeProperty rdf:about="http://example.org/onto/prop/google_data_loss_prevention_job_trigger_sample_method">
    <rdfs:label>sample_method</rdfs:label>
    <rdfs:comment>How to sample rows if not all rows are scanned. Meaningful only when used in conjunction with either
rowsLimit or rowsLimitPercent. If not specified, rows are scanned in the order BigQuery reads them.
If TimespanConfig is set, set this to an empty string to avoid using the default value. Default value: "TOP" Possible values: ["TOP", "RANDOM_START"]</rdfs:comment>
    <rdfs:domain rdf:resource="http://example.org/onto/class/google_data_loss_prevention_job_trigger"/>
    <rdfs:range rdf:resource="http://www.w3.org/2001/XMLSchema#string"/>
  </owl:DatatypeProperty>
  <owl:DatatypeProperty rdf:about="http://example.org/onto/prop/google_data_loss_prevention_job_trigger_name">
    <rdfs:label>name</rdfs:label>
    <rdfs:comment>Name describing the field excluded from scanning.</rdfs:comment>
    <rdfs:domain rdf:resource="http://example.org/onto/class/google_data_loss_prevention_job_trigger"/>
    <rdfs:range rdf:resource="http://www.w3.org/2001/XMLSchema#string"/>
  </owl:DatatypeProperty>
  <owl:DatatypeProperty rdf:about="http://example.org/onto/prop/google_data_loss_prevention_job_trigger_name">
    <rdfs:label>name</rdfs:label>
    <rdfs:comment>Name of a BigQuery field to be returned with the findings.</rdfs:comment>
    <rdfs:domain rdf:resource="http://example.org/onto/class/google_data_loss_prevention_job_trigger"/>
    <rdfs:range rdf:resource="http://www.w3.org/2001/XMLSchema#string"/>
  </owl:DatatypeProperty>
  <owl:DatatypeProperty rdf:about="http://example.org/onto/prop/google_data_loss_prevention_job_trigger_name">
    <rdfs:label>name</rdfs:label>
    <rdfs:comment>Name describing the field to which scanning is limited.</rdfs:comment>
    <rdfs:domain rdf:resource="http://example.org/onto/class/google_data_loss_prevention_job_trigger"/>
    <rdfs:range rdf:resource="http://www.w3.org/2001/XMLSchema#string"/>
  </owl:DatatypeProperty>
  <owl:DatatypeProperty rdf:about="http://example.org/onto/prop/google_data_loss_prevention_job_trigger_dataset_id">
    <rdfs:label>dataset_id</rdfs:label>
    <rdfs:comment>The dataset ID of the table.</rdfs:comment>
    <rdfs:domain rdf:resource="http://example.org/onto/class/google_data_loss_prevention_job_trigger"/>
    <rdfs:range rdf:resource="http://www.w3.org/2001/XMLSchema#string"/>
  </owl:DatatypeProperty>
  <owl:DatatypeProperty rdf:about="http://example.org/onto/prop/google_data_loss_prevention_job_trigger_project_id">
    <rdfs:label>project_id</rdfs:label>
    <rdfs:comment>The Google Cloud Platform project ID of the project containing the table.</rdfs:comment>
    <rdfs:domain rdf:resource="http://example.org/onto/class/google_data_loss_prevention_job_trigger"/>
    <rdfs:range rdf:resource="http://www.w3.org/2001/XMLSchema#string"/>
  </owl:DatatypeProperty>
  <owl:DatatypeProperty rdf:about="http://example.org/onto/prop/google_data_loss_prevention_job_trigger_table_id">
    <rdfs:label>table_id</rdfs:label>
    <rdfs:comment>The name of the table.</rdfs:comment>
    <rdfs:domain rdf:resource="http://example.org/onto/class/google_data_loss_prevention_job_trigger"/>
    <rdfs:range rdf:resource="http://www.w3.org/2001/XMLSchema#string"/>
  </owl:DatatypeProperty>
  <owl:DatatypeProperty rdf:about="http://example.org/onto/prop/google_data_loss_prevention_job_trigger_bytes_limit_per_file">
    <rdfs:label>bytes_limit_per_file</rdfs:label>
    <rdfs:comment>Max number of bytes to scan from a file. If a scanned file's size is bigger than this value
then the rest of the bytes are omitted.</rdfs:comment>
    <rdfs:domain rdf:resource="http://example.org/onto/class/google_data_loss_prevention_job_trigger"/>
    <rdfs:range rdf:resource="http://www.w3.org/2001/XMLSchema#string"/>
  </owl:DatatypeProperty>
  <owl:DatatypeProperty rdf:about="http://example.org/onto/prop/google_data_loss_prevention_job_trigger_bytes_limit_per_file_percent">
    <rdfs:label>bytes_limit_per_file_percent</rdfs:label>
    <rdfs:comment>Max percentage of bytes to scan from a file. The rest are omitted. The number of bytes scanned is rounded down.
Must be between 0 and 100, inclusively. Both 0 and 100 means no limit.</rdfs:comment>
    <rdfs:domain rdf:resource="http://example.org/onto/class/google_data_loss_prevention_job_trigger"/>
    <rdfs:range rdf:resource="http://www.w3.org/2001/XMLSchema#string"/>
  </owl:DatatypeProperty>
  <owl:DatatypeProperty rdf:about="http://example.org/onto/prop/google_data_loss_prevention_job_trigger_file_types">
    <rdfs:label>file_types</rdfs:label>
    <rdfs:comment>List of file type groups to include in the scan. If empty, all files are scanned and available data
format processors are applied. In addition, the binary content of the selected files is always scanned as well.
Images are scanned only as binary if the specified region does not support image inspection and no fileTypes were specified. Possible values: ["BINARY_FILE", "TEXT_FILE", "IMAGE", "WORD", "PDF", "AVRO", "CSV", "TSV", "POWERPOINT", "EXCEL"]</rdfs:comment>
    <rdfs:domain rdf:resource="http://example.org/onto/class/google_data_loss_prevention_job_trigger"/>
    <rdfs:range rdf:resource="http://www.w3.org/2001/XMLSchema#string"/>
  </owl:DatatypeProperty>
  <owl:DatatypeProperty rdf:about="http://example.org/onto/prop/google_data_loss_prevention_job_trigger_files_limit_percent">
    <rdfs:label>files_limit_percent</rdfs:label>
    <rdfs:comment>Limits the number of files to scan to this percentage of the input FileSet. Number of files scanned is rounded down.
Must be between 0 and 100, inclusively. Both 0 and 100 means no limit.</rdfs:comment>
    <rdfs:domain rdf:resource="http://example.org/onto/class/google_data_loss_prevention_job_trigger"/>
    <rdfs:range rdf:resource="http://www.w3.org/2001/XMLSchema#string"/>
  </owl:DatatypeProperty>
  <owl:DatatypeProperty rdf:about="http://example.org/onto/prop/google_data_loss_prevention_job_trigger_sample_method">
    <rdfs:label>sample_method</rdfs:label>
    <rdfs:comment>How to sample bytes if not all bytes are scanned. Meaningful only when used in conjunction with bytesLimitPerFile.
If not specified, scanning would start from the top. Possible values: ["TOP", "RANDOM_START"]</rdfs:comment>
    <rdfs:domain rdf:resource="http://example.org/onto/class/google_data_loss_prevention_job_trigger"/>
    <rdfs:range rdf:resource="http://www.w3.org/2001/XMLSchema#string"/>
  </owl:DatatypeProperty>
  <owl:DatatypeProperty rdf:about="http://example.org/onto/prop/google_data_loss_prevention_job_trigger_url">
    <rdfs:label>url</rdfs:label>
    <rdfs:comment>The Cloud Storage url of the file(s) to scan, in the format 'gs://<bucket>/<path>'. Trailing wildcard
in the path is allowed.

If the url ends in a trailing slash, the bucket or directory represented by the url will be scanned
non-recursively (content in sub-directories will not be scanned). This means that 'gs://mybucket/' is
equivalent to 'gs://mybucket/*', and 'gs://mybucket/directory/' is equivalent to 'gs://mybucket/directory/*'.</rdfs:comment>
    <rdfs:domain rdf:resource="http://example.org/onto/class/google_data_loss_prevention_job_trigger"/>
    <rdfs:range rdf:resource="http://www.w3.org/2001/XMLSchema#string"/>
  </owl:DatatypeProperty>
  <owl:DatatypeProperty rdf:about="http://example.org/onto/prop/google_data_loss_prevention_job_trigger_bucket_name">
    <rdfs:label>bucket_name</rdfs:label>
    <rdfs:comment>The name of a Cloud Storage bucket.</rdfs:comment>
    <rdfs:domain rdf:resource="http://example.org/onto/class/google_data_loss_prevention_job_trigger"/>
    <rdfs:range rdf:resource="http://www.w3.org/2001/XMLSchema#string"/>
  </owl:DatatypeProperty>
  <owl:DatatypeProperty rdf:about="http://example.org/onto/prop/google_data_loss_prevention_job_trigger_exclude_regex">
    <rdfs:label>exclude_regex</rdfs:label>
    <rdfs:comment>A list of regular expressions matching file paths to exclude. All files in the bucket that match at
least one of these regular expressions will be excluded from the scan.</rdfs:comment>
    <rdfs:domain rdf:resource="http://example.org/onto/class/google_data_loss_prevention_job_trigger"/>
    <rdfs:range rdf:resource="http://www.w3.org/2001/XMLSchema#string"/>
  </owl:DatatypeProperty>
  <owl:DatatypeProperty rdf:about="http://example.org/onto/prop/google_data_loss_prevention_job_trigger_include_regex">
    <rdfs:label>include_regex</rdfs:label>
    <rdfs:comment>A list of regular expressions matching file paths to include. All files in the bucket
that match at least one of these regular expressions will be included in the set of files,
except for those that also match an item in excludeRegex. Leaving this field empty will
match all files by default (this is equivalent to including .* in the list)</rdfs:comment>
    <rdfs:domain rdf:resource="http://example.org/onto/class/google_data_loss_prevention_job_trigger"/>
    <rdfs:range rdf:resource="http://www.w3.org/2001/XMLSchema#string"/>
  </owl:DatatypeProperty>
  <owl:DatatypeProperty rdf:about="http://example.org/onto/prop/google_data_loss_prevention_job_trigger_name">
    <rdfs:label>name</rdfs:label>
    <rdfs:comment>The name of the Datastore kind.</rdfs:comment>
    <rdfs:domain rdf:resource="http://example.org/onto/class/google_data_loss_prevention_job_trigger"/>
    <rdfs:range rdf:resource="http://www.w3.org/2001/XMLSchema#string"/>
  </owl:DatatypeProperty>
  <owl:DatatypeProperty rdf:about="http://example.org/onto/prop/google_data_loss_prevention_job_trigger_namespace_id">
    <rdfs:label>namespace_id</rdfs:label>
    <rdfs:comment>If not empty, the ID of the namespace to which the entities belong.</rdfs:comment>
    <rdfs:domain rdf:resource="http://example.org/onto/class/google_data_loss_prevention_job_trigger"/>
    <rdfs:range rdf:resource="http://www.w3.org/2001/XMLSchema#string"/>
  </owl:DatatypeProperty>
  <owl:DatatypeProperty rdf:about="http://example.org/onto/prop/google_data_loss_prevention_job_trigger_project_id">
    <rdfs:label>project_id</rdfs:label>
    <rdfs:comment>The ID of the project to which the entities belong.</rdfs:comment>
    <rdfs:domain rdf:resource="http://example.org/onto/class/google_data_loss_prevention_job_trigger"/>
    <rdfs:range rdf:resource="http://www.w3.org/2001/XMLSchema#string"/>
  </owl:DatatypeProperty>
  <owl:DatatypeProperty rdf:about="http://example.org/onto/prop/google_data_loss_prevention_job_trigger_description">
    <rdfs:label>description</rdfs:label>
    <rdfs:comment>A short description of where the data is coming from. Will be stored once in the job. 256 max length.</rdfs:comment>
    <rdfs:domain rdf:resource="http://example.org/onto/class/google_data_loss_prevention_job_trigger"/>
    <rdfs:range rdf:resource="http://www.w3.org/2001/XMLSchema#string"/>
  </owl:DatatypeProperty>
  <owl:DatatypeProperty rdf:about="http://example.org/onto/prop/google_data_loss_prevention_job_trigger_labels">
    <rdfs:label>labels</rdfs:label>
    <rdfs:comment>To organize findings, these labels will be added to each finding.

Label keys must be between 1 and 63 characters long and must conform to the following regular expression: '[a-z]([-a-z0-9]*[a-z0-9])?'.

Label values must be between 0 and 63 characters long and must conform to the regular expression '([a-z]([-a-z0-9]*[a-z0-9])?)?'.

No more than 10 labels can be associated with a given finding.

Examples:
* '"environment" : "production"'
* '"pipeline" : "etl"'</rdfs:comment>
    <rdfs:domain rdf:resource="http://example.org/onto/class/google_data_loss_prevention_job_trigger"/>
    <rdfs:range rdf:resource="http://www.w3.org/2001/XMLSchema#string"/>
  </owl:DatatypeProperty>
  <owl:DatatypeProperty rdf:about="http://example.org/onto/prop/google_data_loss_prevention_job_trigger_required_finding_label_keys">
    <rdfs:label>required_finding_label_keys</rdfs:label>
    <rdfs:comment>These are labels that each inspection request must include within their 'finding_labels' map. Request
may contain others, but any missing one of these will be rejected.

Label keys must be between 1 and 63 characters long and must conform to the following regular expression: '[a-z]([-a-z0-9]*[a-z0-9])?'.

No more than 10 keys can be required.</rdfs:comment>
    <rdfs:domain rdf:resource="http://example.org/onto/class/google_data_loss_prevention_job_trigger"/>
    <rdfs:range rdf:resource="http://www.w3.org/2001/XMLSchema#string"/>
  </owl:DatatypeProperty>
  <owl:DatatypeProperty rdf:about="http://example.org/onto/prop/google_data_loss_prevention_job_trigger_name">
    <rdfs:label>name</rdfs:label>
    <rdfs:comment>Name describing the field.</rdfs:comment>
    <rdfs:domain rdf:resource="http://example.org/onto/class/google_data_loss_prevention_job_trigger"/>
    <rdfs:range rdf:resource="http://www.w3.org/2001/XMLSchema#string"/>
  </owl:DatatypeProperty>
  <owl:DatatypeProperty rdf:about="http://example.org/onto/prop/google_data_loss_prevention_job_trigger_enable_auto_population_of_timespan_config">
    <rdfs:label>enable_auto_population_of_timespan_config</rdfs:label>
    <rdfs:comment>When the job is started by a JobTrigger we will automatically figure out a valid startTime to avoid
scanning files that have not been modified since the last time the JobTrigger executed. This will
be based on the time of the execution of the last run of the JobTrigger or the timespan endTime
used in the last run of the JobTrigger.</rdfs:comment>
    <rdfs:domain rdf:resource="http://example.org/onto/class/google_data_loss_prevention_job_trigger"/>
    <rdfs:range rdf:resource="http://www.w3.org/2001/XMLSchema#string"/>
  </owl:DatatypeProperty>
  <owl:DatatypeProperty rdf:about="http://example.org/onto/prop/google_data_loss_prevention_job_trigger_end_time">
    <rdfs:label>end_time</rdfs:label>
    <rdfs:comment>Exclude files, tables, or rows newer than this value. If not set, no upper time limit is applied.</rdfs:comment>
    <rdfs:domain rdf:resource="http://example.org/onto/class/google_data_loss_prevention_job_trigger"/>
    <rdfs:range rdf:resource="http://www.w3.org/2001/XMLSchema#string"/>
  </owl:DatatypeProperty>
  <owl:DatatypeProperty rdf:about="http://example.org/onto/prop/google_data_loss_prevention_job_trigger_start_time">
    <rdfs:label>start_time</rdfs:label>
    <rdfs:comment>Exclude files, tables, or rows older than this value. If not set, no lower time limit is applied.</rdfs:comment>
    <rdfs:domain rdf:resource="http://example.org/onto/class/google_data_loss_prevention_job_trigger"/>
    <rdfs:range rdf:resource="http://www.w3.org/2001/XMLSchema#string"/>
  </owl:DatatypeProperty>
  <owl:DatatypeProperty rdf:about="http://example.org/onto/prop/google_data_loss_prevention_job_trigger_name">
    <rdfs:label>name</rdfs:label>
    <rdfs:comment>Specification of the field containing the timestamp of scanned items. Used for data sources like Datastore and BigQuery.

For BigQuery: Required to filter out rows based on the given start and end times. If not specified and the table was
modified between the given start and end times, the entire table will be scanned. The valid data types of the timestamp
field are: INTEGER, DATE, TIMESTAMP, or DATETIME BigQuery column.

For Datastore. Valid data types of the timestamp field are: TIMESTAMP. Datastore entity will be scanned if the
timestamp property does not exist or its value is empty or invalid.</rdfs:comment>
    <rdfs:domain rdf:resource="http://example.org/onto/class/google_data_loss_prevention_job_trigger"/>
    <rdfs:range rdf:resource="http://www.w3.org/2001/XMLSchema#string"/>
  </owl:DatatypeProperty>
  <owl:DatatypeProperty rdf:about="http://example.org/onto/prop/google_data_loss_prevention_job_trigger_create">
    <rdfs:label>create</rdfs:label>
    <rdfs:domain rdf:resource="http://example.org/onto/class/google_data_loss_prevention_job_trigger"/>
    <rdfs:range rdf:resource="http://www.w3.org/2001/XMLSchema#string"/>
  </owl:DatatypeProperty>
  <owl:DatatypeProperty rdf:about="http://example.org/onto/prop/google_data_loss_prevention_job_trigger_delete">
    <rdfs:label>delete</rdfs:label>
    <rdfs:domain rdf:resource="http://example.org/onto/class/google_data_loss_prevention_job_trigger"/>
    <rdfs:range rdf:resource="http://www.w3.org/2001/XMLSchema#string"/>
  </owl:DatatypeProperty>
  <owl:DatatypeProperty rdf:about="http://example.org/onto/prop/google_data_loss_prevention_job_trigger_update">
    <rdfs:label>update</rdfs:label>
    <rdfs:domain rdf:resource="http://example.org/onto/class/google_data_loss_prevention_job_trigger"/>
    <rdfs:range rdf:resource="http://www.w3.org/2001/XMLSchema#string"/>
  </owl:DatatypeProperty>
  <owl:DatatypeProperty rdf:about="http://example.org/onto/prop/google_data_loss_prevention_job_trigger_recurrence_period_duration">
    <rdfs:label>recurrence_period_duration</rdfs:label>
    <rdfs:comment>With this option a job is started a regular periodic basis. For example: every day (86400 seconds).

A scheduled start time will be skipped if the previous execution has not ended when its scheduled time occurs.

This value must be set to a time duration greater than or equal to 1 day and can be no longer than 60 days.

A duration in seconds with up to nine fractional digits, terminated by 's'. Example: "3.5s".</rdfs:comment>
    <rdfs:domain rdf:resource="http://example.org/onto/class/google_data_loss_prevention_job_trigger"/>
    <rdfs:range rdf:resource="http://www.w3.org/2001/XMLSchema#string"/>
  </owl:DatatypeProperty>
</rdf:RDF>
