<?xml version="1.0" encoding="UTF-8"?>
<rdf:RDF
  xmlns:rdf="http://www.w3.org/1999/02/22-rdf-syntax-ns#"
  xmlns:rdfs="http://www.w3.org/2000/01/rdf-schema#"
  xmlns:owl="http://www.w3.org/2002/07/owl#"
  xmlns:xsd="http://www.w3.org/2001/XMLSchema#"
  xml:base="http://example.org/onto/">
  <owl:Class rdf:about="http://example.org/onto/class/google_parallelstore_instance">
    <rdfs:label>google_parallelstore_instance</rdfs:label>
    <rdfs:comment>#
#     ***     AUTO GENERATED CODE    ***    Type: MMv1     ***
#
# ----------------------------------------------------------------------------
#
#     This code is generated by Magic Modules using the following:
#
#     Configuration: https:#github.com/GoogleCloudPlatform/magic-modules/tree/main/mmv1/products/parallelstore/Instance.yaml
#     Template:      https:#github.com/GoogleCloudPlatform/magic-modules/tree/main/mmv1/templates/terraform/resource.html.markdown.tmpl
#
#     DO NOT EDIT this file directly. Any changes made to this file will be
#     overwritten during the next generation cycle.
#
# ----------------------------------------------------------------------------
subcategory: "Parallelstore"
description: |-
  A Parallelstore Instance.
---</rdfs:comment>
  </owl:Class>
  <owl:DatatypeProperty rdf:about="http://example.org/onto/prop/google_parallelstore_instance_access_points">
    <rdfs:label>access_points</rdfs:label>
    <rdfs:comment>Output only. List of access_points.
Contains a list of IPv4 addresses used for client side configuration.</rdfs:comment>
    <rdfs:domain rdf:resource="http://example.org/onto/class/google_parallelstore_instance"/>
    <rdfs:range rdf:resource="http://www.w3.org/2001/XMLSchema#string"/>
  </owl:DatatypeProperty>
  <owl:DatatypeProperty rdf:about="http://example.org/onto/prop/google_parallelstore_instance_capacity_gib">
    <rdfs:label>capacity_gib</rdfs:label>
    <rdfs:comment>Required. Immutable. Storage capacity of Parallelstore instance in Gibibytes (GiB).</rdfs:comment>
    <rdfs:domain rdf:resource="http://example.org/onto/class/google_parallelstore_instance"/>
    <rdfs:range rdf:resource="http://www.w3.org/2001/XMLSchema#string"/>
  </owl:DatatypeProperty>
  <owl:DatatypeProperty rdf:about="http://example.org/onto/prop/google_parallelstore_instance_create_time">
    <rdfs:label>create_time</rdfs:label>
    <rdfs:comment>The time when the instance was created.</rdfs:comment>
    <rdfs:domain rdf:resource="http://example.org/onto/class/google_parallelstore_instance"/>
    <rdfs:range rdf:resource="http://www.w3.org/2001/XMLSchema#string"/>
  </owl:DatatypeProperty>
  <owl:DatatypeProperty rdf:about="http://example.org/onto/prop/google_parallelstore_instance_daos_version">
    <rdfs:label>daos_version</rdfs:label>
    <rdfs:comment>The version of DAOS software running in the instance.</rdfs:comment>
    <rdfs:domain rdf:resource="http://example.org/onto/class/google_parallelstore_instance"/>
    <rdfs:range rdf:resource="http://www.w3.org/2001/XMLSchema#string"/>
  </owl:DatatypeProperty>
  <owl:DatatypeProperty rdf:about="http://example.org/onto/prop/google_parallelstore_instance_deployment_type">
    <rdfs:label>deployment_type</rdfs:label>
    <rdfs:comment>Parallelstore Instance deployment type.
  Possible values:
  DEPLOYMENT_TYPE_UNSPECIFIED
  SCRATCH
  PERSISTENT</rdfs:comment>
    <rdfs:domain rdf:resource="http://example.org/onto/class/google_parallelstore_instance"/>
    <rdfs:range rdf:resource="http://www.w3.org/2001/XMLSchema#string"/>
  </owl:DatatypeProperty>
  <owl:DatatypeProperty rdf:about="http://example.org/onto/prop/google_parallelstore_instance_description">
    <rdfs:label>description</rdfs:label>
    <rdfs:comment>The description of the instance. 2048 characters or less.</rdfs:comment>
    <rdfs:domain rdf:resource="http://example.org/onto/class/google_parallelstore_instance"/>
    <rdfs:range rdf:resource="http://www.w3.org/2001/XMLSchema#string"/>
  </owl:DatatypeProperty>
  <owl:DatatypeProperty rdf:about="http://example.org/onto/prop/google_parallelstore_instance_directory_stripe_level">
    <rdfs:label>directory_stripe_level</rdfs:label>
    <rdfs:comment>Stripe level for directories.
MIN when directory has a small number of files.
MAX when directory has a large number of files.
  Possible values:
  DIRECTORY_STRIPE_LEVEL_UNSPECIFIED
  DIRECTORY_STRIPE_LEVEL_MIN
  DIRECTORY_STRIPE_LEVEL_BALANCED
  DIRECTORY_STRIPE_LEVEL_MAX</rdfs:comment>
    <rdfs:domain rdf:resource="http://example.org/onto/class/google_parallelstore_instance"/>
    <rdfs:range rdf:resource="http://www.w3.org/2001/XMLSchema#string"/>
  </owl:DatatypeProperty>
  <owl:DatatypeProperty rdf:about="http://example.org/onto/prop/google_parallelstore_instance_effective_labels">
    <rdfs:label>effective_labels</rdfs:label>
    <rdfs:comment>All of labels (key/value pairs) present on the resource in GCP, including the labels configured through Terraform, other clients and services.</rdfs:comment>
    <rdfs:domain rdf:resource="http://example.org/onto/class/google_parallelstore_instance"/>
    <rdfs:range rdf:resource="http://www.w3.org/2001/XMLSchema#string"/>
  </owl:DatatypeProperty>
  <owl:DatatypeProperty rdf:about="http://example.org/onto/prop/google_parallelstore_instance_effective_reserved_ip_range">
    <rdfs:label>effective_reserved_ip_range</rdfs:label>
    <rdfs:comment>Immutable. Contains the id of the allocated IP address
range associated with the private service access connection for example, \"test-default\"
associated with IP range 10.0.0.0/29. This field is populated by the service
and contains the value currently used by the service.</rdfs:comment>
    <rdfs:domain rdf:resource="http://example.org/onto/class/google_parallelstore_instance"/>
    <rdfs:range rdf:resource="http://www.w3.org/2001/XMLSchema#string"/>
  </owl:DatatypeProperty>
  <owl:DatatypeProperty rdf:about="http://example.org/onto/prop/google_parallelstore_instance_file_stripe_level">
    <rdfs:label>file_stripe_level</rdfs:label>
    <rdfs:comment>Stripe level for files.
MIN better suited for small size files.
MAX higher throughput performance for larger files.
  Possible values:
  FILE_STRIPE_LEVEL_UNSPECIFIED
  FILE_STRIPE_LEVEL_MIN
  FILE_STRIPE_LEVEL_BALANCED
  FILE_STRIPE_LEVEL_MAX</rdfs:comment>
    <rdfs:domain rdf:resource="http://example.org/onto/class/google_parallelstore_instance"/>
    <rdfs:range rdf:resource="http://www.w3.org/2001/XMLSchema#string"/>
  </owl:DatatypeProperty>
  <owl:DatatypeProperty rdf:about="http://example.org/onto/prop/google_parallelstore_instance_id">
    <rdfs:label>id</rdfs:label>
    <rdfs:domain rdf:resource="http://example.org/onto/class/google_parallelstore_instance"/>
    <rdfs:range rdf:resource="http://www.w3.org/2001/XMLSchema#string"/>
  </owl:DatatypeProperty>
  <owl:DatatypeProperty rdf:about="http://example.org/onto/prop/google_parallelstore_instance_instance_id">
    <rdfs:label>instance_id</rdfs:label>
    <rdfs:comment>The logical name of the Parallelstore instance in the user project with the following restrictions:
  * Must contain only lowercase letters, numbers, and hyphens.
  * Must start with a letter.
  * Must be between 1-63 characters.
  * Must end with a number or a letter.
  * Must be unique within the customer project/ location</rdfs:comment>
    <rdfs:domain rdf:resource="http://example.org/onto/class/google_parallelstore_instance"/>
    <rdfs:range rdf:resource="http://www.w3.org/2001/XMLSchema#string"/>
  </owl:DatatypeProperty>
  <owl:DatatypeProperty rdf:about="http://example.org/onto/prop/google_parallelstore_instance_labels">
    <rdfs:label>labels</rdfs:label>
    <rdfs:comment>Cloud Labels are a flexible and lightweight mechanism for
organizing cloud resources into groups that reflect a customer's organizational
needs and deployment strategies. Cloud Labels can be used to filter collections
of resources. They can be used to control how resource metrics are aggregated.
And they can be used as arguments to policy management rules (e.g. route, firewall,
load balancing, etc.).

* Label keys must be between 1 and 63 characters long and must conform to
 the following regular expression: 'a-z{0,62}'.
* Label values must be between 0 and 63 characters long and must conform
 to the regular expression '[a-z0-9_-]{0,63}'.
* No more than 64 labels can be associated with a given resource.

See https://goo.gl/xmQnxf for more information on and examples of labels.

If you plan to use labels in your own code, please note that additional
characters may be allowed in the future. Therefore, you are advised to use
an internal label representation, such as JSON, which doesn't rely upon
specific characters being disallowed.  For example, representing labels
as the string:  'name + "_" + value' would prove problematic if we were to
allow '"_"' in a future release. "


**Note**: This field is non-authoritative, and will only manage the labels present in your configuration.
Please refer to the field 'effective_labels' for all of the labels present on the resource.</rdfs:comment>
    <rdfs:domain rdf:resource="http://example.org/onto/class/google_parallelstore_instance"/>
    <rdfs:range rdf:resource="http://www.w3.org/2001/XMLSchema#string"/>
  </owl:DatatypeProperty>
  <owl:DatatypeProperty rdf:about="http://example.org/onto/prop/google_parallelstore_instance_location">
    <rdfs:label>location</rdfs:label>
    <rdfs:comment>Part of 'parent'. See documentation of 'projectsId'.</rdfs:comment>
    <rdfs:domain rdf:resource="http://example.org/onto/class/google_parallelstore_instance"/>
    <rdfs:range rdf:resource="http://www.w3.org/2001/XMLSchema#string"/>
  </owl:DatatypeProperty>
  <owl:DatatypeProperty rdf:about="http://example.org/onto/prop/google_parallelstore_instance_name">
    <rdfs:label>name</rdfs:label>
    <rdfs:comment>Identifier. The resource name of the instance, in the format
'projects/{project}/locations/{location}/instances/{instance_id}'</rdfs:comment>
    <rdfs:domain rdf:resource="http://example.org/onto/class/google_parallelstore_instance"/>
    <rdfs:range rdf:resource="http://www.w3.org/2001/XMLSchema#string"/>
  </owl:DatatypeProperty>
  <owl:DatatypeProperty rdf:about="http://example.org/onto/prop/google_parallelstore_instance_network">
    <rdfs:label>network</rdfs:label>
    <rdfs:comment>Immutable. The name of the Google Compute Engine [VPC network](https://cloud.google.com/vpc/docs/vpc)
to which the instance is connected.</rdfs:comment>
    <rdfs:domain rdf:resource="http://example.org/onto/class/google_parallelstore_instance"/>
    <rdfs:range rdf:resource="http://www.w3.org/2001/XMLSchema#string"/>
  </owl:DatatypeProperty>
  <owl:DatatypeProperty rdf:about="http://example.org/onto/prop/google_parallelstore_instance_project">
    <rdfs:label>project</rdfs:label>
    <rdfs:domain rdf:resource="http://example.org/onto/class/google_parallelstore_instance"/>
    <rdfs:range rdf:resource="http://www.w3.org/2001/XMLSchema#string"/>
  </owl:DatatypeProperty>
  <owl:DatatypeProperty rdf:about="http://example.org/onto/prop/google_parallelstore_instance_reserved_ip_range">
    <rdfs:label>reserved_ip_range</rdfs:label>
    <rdfs:comment>Immutable. Contains the id of the allocated IP address range
associated with the private service access connection for example, \"test-default\"
associated with IP range 10.0.0.0/29. If no range id is provided all ranges will
be considered.</rdfs:comment>
    <rdfs:domain rdf:resource="http://example.org/onto/class/google_parallelstore_instance"/>
    <rdfs:range rdf:resource="http://www.w3.org/2001/XMLSchema#string"/>
  </owl:DatatypeProperty>
  <owl:DatatypeProperty rdf:about="http://example.org/onto/prop/google_parallelstore_instance_state">
    <rdfs:label>state</rdfs:label>
    <rdfs:comment>The instance state.
  Possible values:
  STATE_UNSPECIFIED
  CREATING
  ACTIVE
  DELETING
  FAILED
  UPGRADING</rdfs:comment>
    <rdfs:domain rdf:resource="http://example.org/onto/class/google_parallelstore_instance"/>
    <rdfs:range rdf:resource="http://www.w3.org/2001/XMLSchema#string"/>
  </owl:DatatypeProperty>
  <owl:DatatypeProperty rdf:about="http://example.org/onto/prop/google_parallelstore_instance_terraform_labels">
    <rdfs:label>terraform_labels</rdfs:label>
    <rdfs:comment>The combination of labels configured directly on the resource
 and default labels configured on the provider.</rdfs:comment>
    <rdfs:domain rdf:resource="http://example.org/onto/class/google_parallelstore_instance"/>
    <rdfs:range rdf:resource="http://www.w3.org/2001/XMLSchema#string"/>
  </owl:DatatypeProperty>
  <owl:DatatypeProperty rdf:about="http://example.org/onto/prop/google_parallelstore_instance_update_time">
    <rdfs:label>update_time</rdfs:label>
    <rdfs:comment>The time when the instance was updated.</rdfs:comment>
    <rdfs:domain rdf:resource="http://example.org/onto/class/google_parallelstore_instance"/>
    <rdfs:range rdf:resource="http://www.w3.org/2001/XMLSchema#string"/>
  </owl:DatatypeProperty>
  <owl:DatatypeProperty rdf:about="http://example.org/onto/prop/google_parallelstore_instance_create">
    <rdfs:label>create</rdfs:label>
    <rdfs:domain rdf:resource="http://example.org/onto/class/google_parallelstore_instance"/>
    <rdfs:range rdf:resource="http://www.w3.org/2001/XMLSchema#string"/>
  </owl:DatatypeProperty>
  <owl:DatatypeProperty rdf:about="http://example.org/onto/prop/google_parallelstore_instance_delete">
    <rdfs:label>delete</rdfs:label>
    <rdfs:domain rdf:resource="http://example.org/onto/class/google_parallelstore_instance"/>
    <rdfs:range rdf:resource="http://www.w3.org/2001/XMLSchema#string"/>
  </owl:DatatypeProperty>
  <owl:DatatypeProperty rdf:about="http://example.org/onto/prop/google_parallelstore_instance_update">
    <rdfs:label>update</rdfs:label>
    <rdfs:domain rdf:resource="http://example.org/onto/class/google_parallelstore_instance"/>
    <rdfs:range rdf:resource="http://www.w3.org/2001/XMLSchema#string"/>
  </owl:DatatypeProperty>
</rdf:RDF>
