<?xml version="1.0" encoding="UTF-8"?>
<rdf:RDF
  xmlns:rdf="http://www.w3.org/1999/02/22-rdf-syntax-ns#"
  xmlns:rdfs="http://www.w3.org/2000/01/rdf-schema#"
  xmlns:owl="http://www.w3.org/2002/07/owl#"
  xmlns:xsd="http://www.w3.org/2001/XMLSchema#"
  xml:base="http://example.org/onto/">
  <owl:Class rdf:about="http://example.org/onto/class/google_lustre_instance">
    <rdfs:label>google_lustre_instance</rdfs:label>
    <rdfs:comment>#
#     ***     AUTO GENERATED CODE    ***    Type: MMv1     ***
#
# ----------------------------------------------------------------------------
#
#     This code is generated by Magic Modules using the following:
#
#     Configuration: https:#github.com/GoogleCloudPlatform/magic-modules/tree/main/mmv1/products/lustre/Instance.yaml
#     Template:      https:#github.com/GoogleCloudPlatform/magic-modules/tree/main/mmv1/templates/terraform/resource.html.markdown.tmpl
#
#     DO NOT EDIT this file directly. Any changes made to this file will be
#     overwritten during the next generation cycle.
#
# ----------------------------------------------------------------------------
subcategory: "Google Cloud Managed Lustre"
description: |-
  A Managed Lustre instance
---</rdfs:comment>
  </owl:Class>
  <owl:DatatypeProperty rdf:about="http://example.org/onto/prop/google_lustre_instance_capacity_gib">
    <rdfs:label>capacity_gib</rdfs:label>
    <rdfs:comment>The storage capacity of the instance in gibibytes (GiB). Allowed values
are from '18000' to '954000', in increments of 9000.</rdfs:comment>
    <rdfs:domain rdf:resource="http://example.org/onto/class/google_lustre_instance"/>
    <rdfs:range rdf:resource="http://www.w3.org/2001/XMLSchema#string"/>
  </owl:DatatypeProperty>
  <owl:DatatypeProperty rdf:about="http://example.org/onto/prop/google_lustre_instance_create_time">
    <rdfs:label>create_time</rdfs:label>
    <rdfs:comment>Timestamp when the instance was created.</rdfs:comment>
    <rdfs:domain rdf:resource="http://example.org/onto/class/google_lustre_instance"/>
    <rdfs:range rdf:resource="http://www.w3.org/2001/XMLSchema#string"/>
  </owl:DatatypeProperty>
  <owl:DatatypeProperty rdf:about="http://example.org/onto/prop/google_lustre_instance_description">
    <rdfs:label>description</rdfs:label>
    <rdfs:comment>A user-readable description of the instance.</rdfs:comment>
    <rdfs:domain rdf:resource="http://example.org/onto/class/google_lustre_instance"/>
    <rdfs:range rdf:resource="http://www.w3.org/2001/XMLSchema#string"/>
  </owl:DatatypeProperty>
  <owl:DatatypeProperty rdf:about="http://example.org/onto/prop/google_lustre_instance_effective_labels">
    <rdfs:label>effective_labels</rdfs:label>
    <rdfs:comment>All of labels (key/value pairs) present on the resource in GCP, including the labels configured through Terraform, other clients and services.</rdfs:comment>
    <rdfs:domain rdf:resource="http://example.org/onto/class/google_lustre_instance"/>
    <rdfs:range rdf:resource="http://www.w3.org/2001/XMLSchema#string"/>
  </owl:DatatypeProperty>
  <owl:DatatypeProperty rdf:about="http://example.org/onto/prop/google_lustre_instance_filesystem">
    <rdfs:label>filesystem</rdfs:label>
    <rdfs:comment>The filesystem name for this instance. This name is used by client-side
tools, including when mounting the instance. Must be eight characters or
less and can only contain letters and numbers.</rdfs:comment>
    <rdfs:domain rdf:resource="http://example.org/onto/class/google_lustre_instance"/>
    <rdfs:range rdf:resource="http://www.w3.org/2001/XMLSchema#string"/>
  </owl:DatatypeProperty>
  <owl:DatatypeProperty rdf:about="http://example.org/onto/prop/google_lustre_instance_gke_support_enabled">
    <rdfs:label>gke_support_enabled</rdfs:label>
    <rdfs:comment>Indicates whether you want to enable support for GKE clients. By default,
GKE clients are not supported.</rdfs:comment>
    <rdfs:domain rdf:resource="http://example.org/onto/class/google_lustre_instance"/>
    <rdfs:range rdf:resource="http://www.w3.org/2001/XMLSchema#string"/>
  </owl:DatatypeProperty>
  <owl:DatatypeProperty rdf:about="http://example.org/onto/prop/google_lustre_instance_id">
    <rdfs:label>id</rdfs:label>
    <rdfs:domain rdf:resource="http://example.org/onto/class/google_lustre_instance"/>
    <rdfs:range rdf:resource="http://www.w3.org/2001/XMLSchema#string"/>
  </owl:DatatypeProperty>
  <owl:DatatypeProperty rdf:about="http://example.org/onto/prop/google_lustre_instance_instance_id">
    <rdfs:label>instance_id</rdfs:label>
    <rdfs:comment>The name of the Managed Lustre instance.

* Must contain only lowercase letters, numbers, and hyphens.
* Must start with a letter.
* Must be between 1-63 characters.
* Must end with a number or a letter.</rdfs:comment>
    <rdfs:domain rdf:resource="http://example.org/onto/class/google_lustre_instance"/>
    <rdfs:range rdf:resource="http://www.w3.org/2001/XMLSchema#string"/>
  </owl:DatatypeProperty>
  <owl:DatatypeProperty rdf:about="http://example.org/onto/prop/google_lustre_instance_labels">
    <rdfs:label>labels</rdfs:label>
    <rdfs:comment>Labels as key value pairs.

**Note**: This field is non-authoritative, and will only manage the labels present in your configuration.
Please refer to the field 'effective_labels' for all of the labels present on the resource.</rdfs:comment>
    <rdfs:domain rdf:resource="http://example.org/onto/class/google_lustre_instance"/>
    <rdfs:range rdf:resource="http://www.w3.org/2001/XMLSchema#string"/>
  </owl:DatatypeProperty>
  <owl:DatatypeProperty rdf:about="http://example.org/onto/prop/google_lustre_instance_location">
    <rdfs:label>location</rdfs:label>
    <rdfs:comment>Resource ID segment making up resource 'name'. It identifies the resource within its parent collection as described in https://google.aip.dev/122.</rdfs:comment>
    <rdfs:domain rdf:resource="http://example.org/onto/class/google_lustre_instance"/>
    <rdfs:range rdf:resource="http://www.w3.org/2001/XMLSchema#string"/>
  </owl:DatatypeProperty>
  <owl:DatatypeProperty rdf:about="http://example.org/onto/prop/google_lustre_instance_mount_point">
    <rdfs:label>mount_point</rdfs:label>
    <rdfs:comment>Mount point of the instance in the format 'IP_ADDRESS@tcp:/FILESYSTEM'.</rdfs:comment>
    <rdfs:domain rdf:resource="http://example.org/onto/class/google_lustre_instance"/>
    <rdfs:range rdf:resource="http://www.w3.org/2001/XMLSchema#string"/>
  </owl:DatatypeProperty>
  <owl:DatatypeProperty rdf:about="http://example.org/onto/prop/google_lustre_instance_name">
    <rdfs:label>name</rdfs:label>
    <rdfs:comment>Identifier. The name of the instance.</rdfs:comment>
    <rdfs:domain rdf:resource="http://example.org/onto/class/google_lustre_instance"/>
    <rdfs:range rdf:resource="http://www.w3.org/2001/XMLSchema#string"/>
  </owl:DatatypeProperty>
  <owl:DatatypeProperty rdf:about="http://example.org/onto/prop/google_lustre_instance_network">
    <rdfs:label>network</rdfs:label>
    <rdfs:comment>The full name of the VPC network to which the instance is connected.
Must be in the format
'projects/{project_id}/global/networks/{network_name}'.</rdfs:comment>
    <rdfs:domain rdf:resource="http://example.org/onto/class/google_lustre_instance"/>
    <rdfs:range rdf:resource="http://www.w3.org/2001/XMLSchema#string"/>
  </owl:DatatypeProperty>
  <owl:DatatypeProperty rdf:about="http://example.org/onto/prop/google_lustre_instance_per_unit_storage_throughput">
    <rdfs:label>per_unit_storage_throughput</rdfs:label>
    <rdfs:comment>The throughput of the instance in MB/s/TiB.
Valid values are 125, 250, 500, 1000.</rdfs:comment>
    <rdfs:domain rdf:resource="http://example.org/onto/class/google_lustre_instance"/>
    <rdfs:range rdf:resource="http://www.w3.org/2001/XMLSchema#string"/>
  </owl:DatatypeProperty>
  <owl:DatatypeProperty rdf:about="http://example.org/onto/prop/google_lustre_instance_project">
    <rdfs:label>project</rdfs:label>
    <rdfs:domain rdf:resource="http://example.org/onto/class/google_lustre_instance"/>
    <rdfs:range rdf:resource="http://www.w3.org/2001/XMLSchema#string"/>
  </owl:DatatypeProperty>
  <owl:DatatypeProperty rdf:about="http://example.org/onto/prop/google_lustre_instance_state">
    <rdfs:label>state</rdfs:label>
    <rdfs:comment>The state of the instance.
Possible values:
STATE_UNSPECIFIED
ACTIVE
CREATING
DELETING
UPGRADING
REPAIRING
STOPPED</rdfs:comment>
    <rdfs:domain rdf:resource="http://example.org/onto/class/google_lustre_instance"/>
    <rdfs:range rdf:resource="http://www.w3.org/2001/XMLSchema#string"/>
  </owl:DatatypeProperty>
  <owl:DatatypeProperty rdf:about="http://example.org/onto/prop/google_lustre_instance_terraform_labels">
    <rdfs:label>terraform_labels</rdfs:label>
    <rdfs:comment>The combination of labels configured directly on the resource
 and default labels configured on the provider.</rdfs:comment>
    <rdfs:domain rdf:resource="http://example.org/onto/class/google_lustre_instance"/>
    <rdfs:range rdf:resource="http://www.w3.org/2001/XMLSchema#string"/>
  </owl:DatatypeProperty>
  <owl:DatatypeProperty rdf:about="http://example.org/onto/prop/google_lustre_instance_update_time">
    <rdfs:label>update_time</rdfs:label>
    <rdfs:comment>Timestamp when the instance was last updated.</rdfs:comment>
    <rdfs:domain rdf:resource="http://example.org/onto/class/google_lustre_instance"/>
    <rdfs:range rdf:resource="http://www.w3.org/2001/XMLSchema#string"/>
  </owl:DatatypeProperty>
  <owl:DatatypeProperty rdf:about="http://example.org/onto/prop/google_lustre_instance_create">
    <rdfs:label>create</rdfs:label>
    <rdfs:domain rdf:resource="http://example.org/onto/class/google_lustre_instance"/>
    <rdfs:range rdf:resource="http://www.w3.org/2001/XMLSchema#string"/>
  </owl:DatatypeProperty>
  <owl:DatatypeProperty rdf:about="http://example.org/onto/prop/google_lustre_instance_delete">
    <rdfs:label>delete</rdfs:label>
    <rdfs:domain rdf:resource="http://example.org/onto/class/google_lustre_instance"/>
    <rdfs:range rdf:resource="http://www.w3.org/2001/XMLSchema#string"/>
  </owl:DatatypeProperty>
  <owl:DatatypeProperty rdf:about="http://example.org/onto/prop/google_lustre_instance_update">
    <rdfs:label>update</rdfs:label>
    <rdfs:domain rdf:resource="http://example.org/onto/class/google_lustre_instance"/>
    <rdfs:range rdf:resource="http://www.w3.org/2001/XMLSchema#string"/>
  </owl:DatatypeProperty>
</rdf:RDF>
