<?xml version="1.0" encoding="UTF-8"?>
<rdf:RDF
  xmlns:rdf="http://www.w3.org/1999/02/22-rdf-syntax-ns#"
  xmlns:rdfs="http://www.w3.org/2000/01/rdf-schema#"
  xmlns:owl="http://www.w3.org/2002/07/owl#"
  xmlns:xsd="http://www.w3.org/2001/XMLSchema#"
  xml:base="http://example.org/onto/">
  <owl:Class rdf:about="http://example.org/onto/class/google_service_networking_vpc_service_controls">
    <rdfs:label>google_service_networking_vpc_service_controls</rdfs:label>
    <rdfs:comment>#
#     ***     AUTO GENERATED CODE    ***    Type: MMv1     ***
#
# ----------------------------------------------------------------------------
#
#     This code is generated by Magic Modules using the following:
#
#     Configuration: https:#github.com/GoogleCloudPlatform/magic-modules/tree/main/mmv1/products/servicenetworking/VPCServiceControls.yaml
#     Template:      https:#github.com/GoogleCloudPlatform/magic-modules/tree/main/mmv1/templates/terraform/resource.html.markdown.tmpl
#
#     DO NOT EDIT this file directly. Any changes made to this file will be
#     overwritten during the next generation cycle.
#
# ----------------------------------------------------------------------------
subcategory: "Service Networking"
description: |-
  Manages the VPC Service Controls configuration for a service
  networking connection
  When enabled, Google Cloud makes the following
  route configuration changes in the service producer VPC network:
  - Removes the IPv4 default route (destination 0.
---</rdfs:comment>
  </owl:Class>
  <owl:DatatypeProperty rdf:about="http://example.org/onto/prop/google_service_networking_vpc_service_controls_enabled">
    <rdfs:label>enabled</rdfs:label>
    <rdfs:comment>Desired VPC Service Controls state service producer VPC network, as
described at the top of this page.</rdfs:comment>
    <rdfs:domain rdf:resource="http://example.org/onto/class/google_service_networking_vpc_service_controls"/>
    <rdfs:range rdf:resource="http://www.w3.org/2001/XMLSchema#string"/>
  </owl:DatatypeProperty>
  <owl:DatatypeProperty rdf:about="http://example.org/onto/prop/google_service_networking_vpc_service_controls_id">
    <rdfs:label>id</rdfs:label>
    <rdfs:domain rdf:resource="http://example.org/onto/class/google_service_networking_vpc_service_controls"/>
    <rdfs:range rdf:resource="http://www.w3.org/2001/XMLSchema#string"/>
  </owl:DatatypeProperty>
  <owl:DatatypeProperty rdf:about="http://example.org/onto/prop/google_service_networking_vpc_service_controls_network">
    <rdfs:label>network</rdfs:label>
    <rdfs:comment>The network that the consumer is using to connect with services.</rdfs:comment>
    <rdfs:domain rdf:resource="http://example.org/onto/class/google_service_networking_vpc_service_controls"/>
    <rdfs:range rdf:resource="http://www.w3.org/2001/XMLSchema#string"/>
  </owl:DatatypeProperty>
  <owl:DatatypeProperty rdf:about="http://example.org/onto/prop/google_service_networking_vpc_service_controls_project">
    <rdfs:label>project</rdfs:label>
    <rdfs:comment>The id of the Google Cloud project containing the consumer network.</rdfs:comment>
    <rdfs:domain rdf:resource="http://example.org/onto/class/google_service_networking_vpc_service_controls"/>
    <rdfs:range rdf:resource="http://www.w3.org/2001/XMLSchema#string"/>
  </owl:DatatypeProperty>
  <owl:DatatypeProperty rdf:about="http://example.org/onto/prop/google_service_networking_vpc_service_controls_service">
    <rdfs:label>service</rdfs:label>
    <rdfs:comment>The service that is managing peering connectivity for a service
producer's organization. For Google services that support this
functionality, this value is 'servicenetworking.googleapis.com'.</rdfs:comment>
    <rdfs:domain rdf:resource="http://example.org/onto/class/google_service_networking_vpc_service_controls"/>
    <rdfs:range rdf:resource="http://www.w3.org/2001/XMLSchema#string"/>
  </owl:DatatypeProperty>
  <owl:DatatypeProperty rdf:about="http://example.org/onto/prop/google_service_networking_vpc_service_controls_create">
    <rdfs:label>create</rdfs:label>
    <rdfs:domain rdf:resource="http://example.org/onto/class/google_service_networking_vpc_service_controls"/>
    <rdfs:range rdf:resource="http://www.w3.org/2001/XMLSchema#string"/>
  </owl:DatatypeProperty>
  <owl:DatatypeProperty rdf:about="http://example.org/onto/prop/google_service_networking_vpc_service_controls_delete">
    <rdfs:label>delete</rdfs:label>
    <rdfs:domain rdf:resource="http://example.org/onto/class/google_service_networking_vpc_service_controls"/>
    <rdfs:range rdf:resource="http://www.w3.org/2001/XMLSchema#string"/>
  </owl:DatatypeProperty>
  <owl:DatatypeProperty rdf:about="http://example.org/onto/prop/google_service_networking_vpc_service_controls_update">
    <rdfs:label>update</rdfs:label>
    <rdfs:domain rdf:resource="http://example.org/onto/class/google_service_networking_vpc_service_controls"/>
    <rdfs:range rdf:resource="http://www.w3.org/2001/XMLSchema#string"/>
  </owl:DatatypeProperty>
</rdf:RDF>
