<?xml version="1.0" encoding="UTF-8"?>
<rdf:RDF
  xmlns:rdf="http://www.w3.org/1999/02/22-rdf-syntax-ns#"
  xmlns:rdfs="http://www.w3.org/2000/01/rdf-schema#"
  xmlns:owl="http://www.w3.org/2002/07/owl#"
  xmlns:xsd="http://www.w3.org/2001/XMLSchema#"
  xml:base="http://example.org/onto/">
  <owl:Class rdf:about="http://example.org/onto/class/google_iam_oauth_client">
    <rdfs:label>google_iam_oauth_client</rdfs:label>
    <rdfs:comment>#
#     ***     AUTO GENERATED CODE    ***    Type: MMv1     ***
#
# ----------------------------------------------------------------------------
#
#     This code is generated by Magic Modules using the following:
#
#     Configuration: https:#github.com/GoogleCloudPlatform/magic-modules/tree/main/mmv1/products/iamworkforcepool/OauthClient.yaml
#     Template:      https:#github.com/GoogleCloudPlatform/magic-modules/tree/main/mmv1/templates/terraform/resource.html.markdown.tmpl
#
#     DO NOT EDIT this file directly. Any changes made to this file will be
#     overwritten during the next generation cycle.
#
# ----------------------------------------------------------------------------
subcategory: "Cloud IAM"
description: |-
  Represents an OAuth Client.
---</rdfs:comment>
  </owl:Class>
  <owl:DatatypeProperty rdf:about="http://example.org/onto/prop/google_iam_oauth_client_allowed_grant_types">
    <rdfs:label>allowed_grant_types</rdfs:label>
    <rdfs:comment>Required. The list of OAuth grant types is allowed for the OauthClient.</rdfs:comment>
    <rdfs:domain rdf:resource="http://example.org/onto/class/google_iam_oauth_client"/>
    <rdfs:range rdf:resource="http://www.w3.org/2001/XMLSchema#string"/>
  </owl:DatatypeProperty>
  <owl:DatatypeProperty rdf:about="http://example.org/onto/prop/google_iam_oauth_client_allowed_redirect_uris">
    <rdfs:label>allowed_redirect_uris</rdfs:label>
    <rdfs:comment>Required. The list of redirect uris that is allowed to redirect back
when authorization process is completed.</rdfs:comment>
    <rdfs:domain rdf:resource="http://example.org/onto/class/google_iam_oauth_client"/>
    <rdfs:range rdf:resource="http://www.w3.org/2001/XMLSchema#string"/>
  </owl:DatatypeProperty>
  <owl:DatatypeProperty rdf:about="http://example.org/onto/prop/google_iam_oauth_client_allowed_scopes">
    <rdfs:label>allowed_scopes</rdfs:label>
    <rdfs:comment>Required. The list of scopes that the OauthClient is allowed to request during
OAuth flows.

The following scopes are supported:

* 'https://www.googleapis.com/auth/cloud-platform': See, edit, configure,
and delete your Google Cloud data and see the email address for your Google
Account.
* 'openid': The OAuth client can associate you with your personal
information on Google Cloud.
* 'email': The OAuth client can read a federated identity's email address.
* 'groups': The OAuth client can read a federated identity's groups.</rdfs:comment>
    <rdfs:domain rdf:resource="http://example.org/onto/class/google_iam_oauth_client"/>
    <rdfs:range rdf:resource="http://www.w3.org/2001/XMLSchema#string"/>
  </owl:DatatypeProperty>
  <owl:DatatypeProperty rdf:about="http://example.org/onto/prop/google_iam_oauth_client_client_id">
    <rdfs:label>client_id</rdfs:label>
    <rdfs:comment>Output only. The system-generated OauthClient id.</rdfs:comment>
    <rdfs:domain rdf:resource="http://example.org/onto/class/google_iam_oauth_client"/>
    <rdfs:range rdf:resource="http://www.w3.org/2001/XMLSchema#string"/>
  </owl:DatatypeProperty>
  <owl:DatatypeProperty rdf:about="http://example.org/onto/prop/google_iam_oauth_client_client_type">
    <rdfs:label>client_type</rdfs:label>
    <rdfs:comment>Immutable. The type of OauthClient. Either public or private.
For private clients, the client secret can be managed using the dedicated
OauthClientCredential resource.
Possible values:
CLIENT_TYPE_UNSPECIFIED
PUBLIC_CLIENT
CONFIDENTIAL_CLIENT</rdfs:comment>
    <rdfs:domain rdf:resource="http://example.org/onto/class/google_iam_oauth_client"/>
    <rdfs:range rdf:resource="http://www.w3.org/2001/XMLSchema#string"/>
  </owl:DatatypeProperty>
  <owl:DatatypeProperty rdf:about="http://example.org/onto/prop/google_iam_oauth_client_description">
    <rdfs:label>description</rdfs:label>
    <rdfs:comment>A user-specified description of the OauthClient.

Cannot exceed 256 characters.</rdfs:comment>
    <rdfs:domain rdf:resource="http://example.org/onto/class/google_iam_oauth_client"/>
    <rdfs:range rdf:resource="http://www.w3.org/2001/XMLSchema#string"/>
  </owl:DatatypeProperty>
  <owl:DatatypeProperty rdf:about="http://example.org/onto/prop/google_iam_oauth_client_disabled">
    <rdfs:label>disabled</rdfs:label>
    <rdfs:comment>Whether the OauthClient is disabled. You cannot use a disabled OAuth
client.</rdfs:comment>
    <rdfs:domain rdf:resource="http://example.org/onto/class/google_iam_oauth_client"/>
    <rdfs:range rdf:resource="http://www.w3.org/2001/XMLSchema#string"/>
  </owl:DatatypeProperty>
  <owl:DatatypeProperty rdf:about="http://example.org/onto/prop/google_iam_oauth_client_display_name">
    <rdfs:label>display_name</rdfs:label>
    <rdfs:comment>A user-specified display name of the OauthClient.

Cannot exceed 32 characters.</rdfs:comment>
    <rdfs:domain rdf:resource="http://example.org/onto/class/google_iam_oauth_client"/>
    <rdfs:range rdf:resource="http://www.w3.org/2001/XMLSchema#string"/>
  </owl:DatatypeProperty>
  <owl:DatatypeProperty rdf:about="http://example.org/onto/prop/google_iam_oauth_client_expire_time">
    <rdfs:label>expire_time</rdfs:label>
    <rdfs:comment>Time after which the OauthClient will be permanently purged and cannot
be recovered.</rdfs:comment>
    <rdfs:domain rdf:resource="http://example.org/onto/class/google_iam_oauth_client"/>
    <rdfs:range rdf:resource="http://www.w3.org/2001/XMLSchema#string"/>
  </owl:DatatypeProperty>
  <owl:DatatypeProperty rdf:about="http://example.org/onto/prop/google_iam_oauth_client_id">
    <rdfs:label>id</rdfs:label>
    <rdfs:domain rdf:resource="http://example.org/onto/class/google_iam_oauth_client"/>
    <rdfs:range rdf:resource="http://www.w3.org/2001/XMLSchema#string"/>
  </owl:DatatypeProperty>
  <owl:DatatypeProperty rdf:about="http://example.org/onto/prop/google_iam_oauth_client_location">
    <rdfs:label>location</rdfs:label>
    <rdfs:comment>Resource ID segment making up resource 'name'. It identifies the resource within its parent collection as described in https://google.aip.dev/122.</rdfs:comment>
    <rdfs:domain rdf:resource="http://example.org/onto/class/google_iam_oauth_client"/>
    <rdfs:range rdf:resource="http://www.w3.org/2001/XMLSchema#string"/>
  </owl:DatatypeProperty>
  <owl:DatatypeProperty rdf:about="http://example.org/onto/prop/google_iam_oauth_client_name">
    <rdfs:label>name</rdfs:label>
    <rdfs:comment>Immutable. Identifier. The resource name of the OauthClient.

Format:'projects/{project}/locations/{location}/oauthClients/{oauth_client}'.</rdfs:comment>
    <rdfs:domain rdf:resource="http://example.org/onto/class/google_iam_oauth_client"/>
    <rdfs:range rdf:resource="http://www.w3.org/2001/XMLSchema#string"/>
  </owl:DatatypeProperty>
  <owl:DatatypeProperty rdf:about="http://example.org/onto/prop/google_iam_oauth_client_oauth_client_id">
    <rdfs:label>oauth_client_id</rdfs:label>
    <rdfs:comment>Required. The ID to use for the OauthClient, which becomes the final component of
the resource name. This value should be a string of 6 to 63 lowercase
letters, digits, or hyphens. It must start with a letter, and cannot have a
trailing hyphen. The prefix 'gcp-' is reserved for use by Google, and may
not be specified.</rdfs:comment>
    <rdfs:domain rdf:resource="http://example.org/onto/class/google_iam_oauth_client"/>
    <rdfs:range rdf:resource="http://www.w3.org/2001/XMLSchema#string"/>
  </owl:DatatypeProperty>
  <owl:DatatypeProperty rdf:about="http://example.org/onto/prop/google_iam_oauth_client_project">
    <rdfs:label>project</rdfs:label>
    <rdfs:domain rdf:resource="http://example.org/onto/class/google_iam_oauth_client"/>
    <rdfs:range rdf:resource="http://www.w3.org/2001/XMLSchema#string"/>
  </owl:DatatypeProperty>
  <owl:DatatypeProperty rdf:about="http://example.org/onto/prop/google_iam_oauth_client_state">
    <rdfs:label>state</rdfs:label>
    <rdfs:comment>The state of the OauthClient.
Possible values:
STATE_UNSPECIFIED
ACTIVE
DELETED</rdfs:comment>
    <rdfs:domain rdf:resource="http://example.org/onto/class/google_iam_oauth_client"/>
    <rdfs:range rdf:resource="http://www.w3.org/2001/XMLSchema#string"/>
  </owl:DatatypeProperty>
  <owl:DatatypeProperty rdf:about="http://example.org/onto/prop/google_iam_oauth_client_create">
    <rdfs:label>create</rdfs:label>
    <rdfs:domain rdf:resource="http://example.org/onto/class/google_iam_oauth_client"/>
    <rdfs:range rdf:resource="http://www.w3.org/2001/XMLSchema#string"/>
  </owl:DatatypeProperty>
  <owl:DatatypeProperty rdf:about="http://example.org/onto/prop/google_iam_oauth_client_delete">
    <rdfs:label>delete</rdfs:label>
    <rdfs:domain rdf:resource="http://example.org/onto/class/google_iam_oauth_client"/>
    <rdfs:range rdf:resource="http://www.w3.org/2001/XMLSchema#string"/>
  </owl:DatatypeProperty>
  <owl:DatatypeProperty rdf:about="http://example.org/onto/prop/google_iam_oauth_client_update">
    <rdfs:label>update</rdfs:label>
    <rdfs:domain rdf:resource="http://example.org/onto/class/google_iam_oauth_client"/>
    <rdfs:range rdf:resource="http://www.w3.org/2001/XMLSchema#string"/>
  </owl:DatatypeProperty>
</rdf:RDF>
