<?xml version="1.0" encoding="UTF-8"?>
<rdf:RDF
  xmlns:rdf="http://www.w3.org/1999/02/22-rdf-syntax-ns#"
  xmlns:rdfs="http://www.w3.org/2000/01/rdf-schema#"
  xmlns:owl="http://www.w3.org/2002/07/owl#"
  xmlns:xsd="http://www.w3.org/2001/XMLSchema#"
  xml:base="http://example.org/onto/">
  <owl:Class rdf:about="http://example.org/onto/class/google_backup_dr_backup_plan">
    <rdfs:label>google_backup_dr_backup_plan</rdfs:label>
    <rdfs:comment>#
#     ***     AUTO GENERATED CODE    ***    Type: MMv1     ***
#
# ----------------------------------------------------------------------------
#
#     This code is generated by Magic Modules using the following:
#
#     Configuration: https:#github.com/GoogleCloudPlatform/magic-modules/tree/main/mmv1/products/backupdr/BackupPlan.yaml
#     Template:      https:#github.com/GoogleCloudPlatform/magic-modules/tree/main/mmv1/templates/terraform/resource.html.markdown.tmpl
#
#     DO NOT EDIT this file directly. Any changes made to this file will be
#     overwritten during the next generation cycle.
#
# ----------------------------------------------------------------------------
subcategory: "Backup and DR Service"
description: |-
  A backup plan defines when and how to back up a resource, including the backup's schedule, retention, and location.
---</rdfs:comment>
  </owl:Class>
  <owl:DatatypeProperty rdf:about="http://example.org/onto/prop/google_backup_dr_backup_plan_backup_plan_id">
    <rdfs:label>backup_plan_id</rdfs:label>
    <rdfs:comment>The ID of the backup plan</rdfs:comment>
    <rdfs:domain rdf:resource="http://example.org/onto/class/google_backup_dr_backup_plan"/>
    <rdfs:range rdf:resource="http://www.w3.org/2001/XMLSchema#string"/>
  </owl:DatatypeProperty>
  <owl:DatatypeProperty rdf:about="http://example.org/onto/prop/google_backup_dr_backup_plan_backup_vault">
    <rdfs:label>backup_vault</rdfs:label>
    <rdfs:comment>Backup vault where the backups gets stored using this Backup plan.</rdfs:comment>
    <rdfs:domain rdf:resource="http://example.org/onto/class/google_backup_dr_backup_plan"/>
    <rdfs:range rdf:resource="http://www.w3.org/2001/XMLSchema#string"/>
  </owl:DatatypeProperty>
  <owl:DatatypeProperty rdf:about="http://example.org/onto/prop/google_backup_dr_backup_plan_backup_vault_service_account">
    <rdfs:label>backup_vault_service_account</rdfs:label>
    <rdfs:comment>The Google Cloud Platform Service Account to be used by the BackupVault for taking backups.</rdfs:comment>
    <rdfs:domain rdf:resource="http://example.org/onto/class/google_backup_dr_backup_plan"/>
    <rdfs:range rdf:resource="http://www.w3.org/2001/XMLSchema#string"/>
  </owl:DatatypeProperty>
  <owl:DatatypeProperty rdf:about="http://example.org/onto/prop/google_backup_dr_backup_plan_create_time">
    <rdfs:label>create_time</rdfs:label>
    <rdfs:comment>When the 'BackupPlan' was created.</rdfs:comment>
    <rdfs:domain rdf:resource="http://example.org/onto/class/google_backup_dr_backup_plan"/>
    <rdfs:range rdf:resource="http://www.w3.org/2001/XMLSchema#string"/>
  </owl:DatatypeProperty>
  <owl:DatatypeProperty rdf:about="http://example.org/onto/prop/google_backup_dr_backup_plan_description">
    <rdfs:label>description</rdfs:label>
    <rdfs:comment>The description allows for additional details about 'BackupPlan' and its use cases to be provided.</rdfs:comment>
    <rdfs:domain rdf:resource="http://example.org/onto/class/google_backup_dr_backup_plan"/>
    <rdfs:range rdf:resource="http://www.w3.org/2001/XMLSchema#string"/>
  </owl:DatatypeProperty>
  <owl:DatatypeProperty rdf:about="http://example.org/onto/prop/google_backup_dr_backup_plan_id">
    <rdfs:label>id</rdfs:label>
    <rdfs:domain rdf:resource="http://example.org/onto/class/google_backup_dr_backup_plan"/>
    <rdfs:range rdf:resource="http://www.w3.org/2001/XMLSchema#string"/>
  </owl:DatatypeProperty>
  <owl:DatatypeProperty rdf:about="http://example.org/onto/prop/google_backup_dr_backup_plan_location">
    <rdfs:label>location</rdfs:label>
    <rdfs:comment>The location for the backup plan</rdfs:comment>
    <rdfs:domain rdf:resource="http://example.org/onto/class/google_backup_dr_backup_plan"/>
    <rdfs:range rdf:resource="http://www.w3.org/2001/XMLSchema#string"/>
  </owl:DatatypeProperty>
  <owl:DatatypeProperty rdf:about="http://example.org/onto/prop/google_backup_dr_backup_plan_log_retention_days">
    <rdfs:label>log_retention_days</rdfs:label>
    <rdfs:comment>This is only applicable for CloudSql resource. Days for which logs will be stored. This value should be greater than or equal to minimum enforced log retention duration of the backup vault.</rdfs:comment>
    <rdfs:domain rdf:resource="http://example.org/onto/class/google_backup_dr_backup_plan"/>
    <rdfs:range rdf:resource="http://www.w3.org/2001/XMLSchema#string"/>
  </owl:DatatypeProperty>
  <owl:DatatypeProperty rdf:about="http://example.org/onto/prop/google_backup_dr_backup_plan_name">
    <rdfs:label>name</rdfs:label>
    <rdfs:comment>The name of backup plan resource created</rdfs:comment>
    <rdfs:domain rdf:resource="http://example.org/onto/class/google_backup_dr_backup_plan"/>
    <rdfs:range rdf:resource="http://www.w3.org/2001/XMLSchema#string"/>
  </owl:DatatypeProperty>
  <owl:DatatypeProperty rdf:about="http://example.org/onto/prop/google_backup_dr_backup_plan_project">
    <rdfs:label>project</rdfs:label>
    <rdfs:domain rdf:resource="http://example.org/onto/class/google_backup_dr_backup_plan"/>
    <rdfs:range rdf:resource="http://www.w3.org/2001/XMLSchema#string"/>
  </owl:DatatypeProperty>
  <owl:DatatypeProperty rdf:about="http://example.org/onto/prop/google_backup_dr_backup_plan_resource_type">
    <rdfs:label>resource_type</rdfs:label>
    <rdfs:comment>The resource type to which the 'BackupPlan' will be applied.
Examples include, "compute.googleapis.com/Instance", "compute.googleapis.com/Disk", "sqladmin.googleapis.com/Instance" and "storage.googleapis.com/Bucket".</rdfs:comment>
    <rdfs:domain rdf:resource="http://example.org/onto/class/google_backup_dr_backup_plan"/>
    <rdfs:range rdf:resource="http://www.w3.org/2001/XMLSchema#string"/>
  </owl:DatatypeProperty>
  <owl:DatatypeProperty rdf:about="http://example.org/onto/prop/google_backup_dr_backup_plan_supported_resource_types">
    <rdfs:label>supported_resource_types</rdfs:label>
    <rdfs:comment>The list of all resource types to which the 'BackupPlan' can be applied.</rdfs:comment>
    <rdfs:domain rdf:resource="http://example.org/onto/class/google_backup_dr_backup_plan"/>
    <rdfs:range rdf:resource="http://www.w3.org/2001/XMLSchema#string"/>
  </owl:DatatypeProperty>
  <owl:DatatypeProperty rdf:about="http://example.org/onto/prop/google_backup_dr_backup_plan_update_time">
    <rdfs:label>update_time</rdfs:label>
    <rdfs:comment>When the 'BackupPlan' was last updated.</rdfs:comment>
    <rdfs:domain rdf:resource="http://example.org/onto/class/google_backup_dr_backup_plan"/>
    <rdfs:range rdf:resource="http://www.w3.org/2001/XMLSchema#string"/>
  </owl:DatatypeProperty>
  <owl:DatatypeProperty rdf:about="http://example.org/onto/prop/google_backup_dr_backup_plan_backup_retention_days">
    <rdfs:label>backup_retention_days</rdfs:label>
    <rdfs:comment>Configures the duration for which backup data will be kept. The value should be greater than or equal to minimum enforced retention of the backup vault.</rdfs:comment>
    <rdfs:domain rdf:resource="http://example.org/onto/class/google_backup_dr_backup_plan"/>
    <rdfs:range rdf:resource="http://www.w3.org/2001/XMLSchema#string"/>
  </owl:DatatypeProperty>
  <owl:DatatypeProperty rdf:about="http://example.org/onto/prop/google_backup_dr_backup_plan_rule_id">
    <rdfs:label>rule_id</rdfs:label>
    <rdfs:comment>The unique ID of this 'BackupRule'. The 'rule_id' is unique per 'BackupPlan'.</rdfs:comment>
    <rdfs:domain rdf:resource="http://example.org/onto/class/google_backup_dr_backup_plan"/>
    <rdfs:range rdf:resource="http://www.w3.org/2001/XMLSchema#string"/>
  </owl:DatatypeProperty>
  <owl:DatatypeProperty rdf:about="http://example.org/onto/prop/google_backup_dr_backup_plan_days_of_month">
    <rdfs:label>days_of_month</rdfs:label>
    <rdfs:comment>Specifies days of months like 1, 5, or 14 on which jobs will run.</rdfs:comment>
    <rdfs:domain rdf:resource="http://example.org/onto/class/google_backup_dr_backup_plan"/>
    <rdfs:range rdf:resource="http://www.w3.org/2001/XMLSchema#string"/>
  </owl:DatatypeProperty>
  <owl:DatatypeProperty rdf:about="http://example.org/onto/prop/google_backup_dr_backup_plan_days_of_week">
    <rdfs:label>days_of_week</rdfs:label>
    <rdfs:comment>Specifies days of week like MONDAY or TUESDAY, on which jobs will run. This is required for 'recurrence_type', 'WEEKLY' and is not applicable otherwise. Possible values: ["DAY_OF_WEEK_UNSPECIFIED", "MONDAY", "TUESDAY", "WEDNESDAY", "THURSDAY", "FRIDAY", "SATURDAY", "SUNDAY"]</rdfs:comment>
    <rdfs:domain rdf:resource="http://example.org/onto/class/google_backup_dr_backup_plan"/>
    <rdfs:range rdf:resource="http://www.w3.org/2001/XMLSchema#string"/>
  </owl:DatatypeProperty>
  <owl:DatatypeProperty rdf:about="http://example.org/onto/prop/google_backup_dr_backup_plan_hourly_frequency">
    <rdfs:label>hourly_frequency</rdfs:label>
    <rdfs:comment>Specifies frequency for hourly backups. An hourly frequency of 2 means jobs will run every 2 hours from start time till end time defined.
This is required for 'recurrence_type', 'HOURLY' and is not applicable otherwise.</rdfs:comment>
    <rdfs:domain rdf:resource="http://example.org/onto/class/google_backup_dr_backup_plan"/>
    <rdfs:range rdf:resource="http://www.w3.org/2001/XMLSchema#string"/>
  </owl:DatatypeProperty>
  <owl:DatatypeProperty rdf:about="http://example.org/onto/prop/google_backup_dr_backup_plan_months">
    <rdfs:label>months</rdfs:label>
    <rdfs:comment>Specifies values of months Possible values: ["MONTH_UNSPECIFIED", "JANUARY", "FEBRUARY", "MARCH", "APRIL", "MAY", "JUNE", "JULY", "AUGUST", "SEPTEMBER", "OCTOBER", "NOVEMBER", "DECEMBER"]</rdfs:comment>
    <rdfs:domain rdf:resource="http://example.org/onto/class/google_backup_dr_backup_plan"/>
    <rdfs:range rdf:resource="http://www.w3.org/2001/XMLSchema#string"/>
  </owl:DatatypeProperty>
  <owl:DatatypeProperty rdf:about="http://example.org/onto/prop/google_backup_dr_backup_plan_recurrence_type">
    <rdfs:label>recurrence_type</rdfs:label>
    <rdfs:comment>RecurrenceType enumerates the applicable periodicity for the schedule. Possible values: ["HOURLY", "DAILY", "WEEKLY", "MONTHLY", "YEARLY"]</rdfs:comment>
    <rdfs:domain rdf:resource="http://example.org/onto/class/google_backup_dr_backup_plan"/>
    <rdfs:range rdf:resource="http://www.w3.org/2001/XMLSchema#string"/>
  </owl:DatatypeProperty>
  <owl:DatatypeProperty rdf:about="http://example.org/onto/prop/google_backup_dr_backup_plan_time_zone">
    <rdfs:label>time_zone</rdfs:label>
    <rdfs:comment>The time zone to be used when interpreting the schedule.</rdfs:comment>
    <rdfs:domain rdf:resource="http://example.org/onto/class/google_backup_dr_backup_plan"/>
    <rdfs:range rdf:resource="http://www.w3.org/2001/XMLSchema#string"/>
  </owl:DatatypeProperty>
  <owl:DatatypeProperty rdf:about="http://example.org/onto/prop/google_backup_dr_backup_plan_end_hour_of_day">
    <rdfs:label>end_hour_of_day</rdfs:label>
    <rdfs:comment>The hour of the day (1-24) when the window ends, for example, if the value of end hour of the day is 10, that means the backup window end time is 10:00.
The end hour of the day should be greater than the start</rdfs:comment>
    <rdfs:domain rdf:resource="http://example.org/onto/class/google_backup_dr_backup_plan"/>
    <rdfs:range rdf:resource="http://www.w3.org/2001/XMLSchema#string"/>
  </owl:DatatypeProperty>
  <owl:DatatypeProperty rdf:about="http://example.org/onto/prop/google_backup_dr_backup_plan_start_hour_of_day">
    <rdfs:label>start_hour_of_day</rdfs:label>
    <rdfs:comment>The hour of the day (0-23) when the window starts, for example, if the value of the start hour of the day is 6, that means the backup window starts at 6:00.</rdfs:comment>
    <rdfs:domain rdf:resource="http://example.org/onto/class/google_backup_dr_backup_plan"/>
    <rdfs:range rdf:resource="http://www.w3.org/2001/XMLSchema#string"/>
  </owl:DatatypeProperty>
  <owl:DatatypeProperty rdf:about="http://example.org/onto/prop/google_backup_dr_backup_plan_day_of_week">
    <rdfs:label>day_of_week</rdfs:label>
    <rdfs:comment>Specifies the day of the week. Possible values: ["DAY_OF_WEEK_UNSPECIFIED", "MONDAY", "TUESDAY", "WEDNESDAY", "THURSDAY", "FRIDAY", "SATURDAY", "SUNDAY"]</rdfs:comment>
    <rdfs:domain rdf:resource="http://example.org/onto/class/google_backup_dr_backup_plan"/>
    <rdfs:range rdf:resource="http://www.w3.org/2001/XMLSchema#string"/>
  </owl:DatatypeProperty>
  <owl:DatatypeProperty rdf:about="http://example.org/onto/prop/google_backup_dr_backup_plan_week_of_month">
    <rdfs:label>week_of_month</rdfs:label>
    <rdfs:comment>WeekOfMonth enumerates possible weeks in the month, e.g. the first, third, or last week of the month. Possible values: ["WEEK_OF_MONTH_UNSPECIFIED", "FIRST", "SECOND", "THIRD", "FOURTH", "LAST"]</rdfs:comment>
    <rdfs:domain rdf:resource="http://example.org/onto/class/google_backup_dr_backup_plan"/>
    <rdfs:range rdf:resource="http://www.w3.org/2001/XMLSchema#string"/>
  </owl:DatatypeProperty>
  <owl:DatatypeProperty rdf:about="http://example.org/onto/prop/google_backup_dr_backup_plan_create">
    <rdfs:label>create</rdfs:label>
    <rdfs:domain rdf:resource="http://example.org/onto/class/google_backup_dr_backup_plan"/>
    <rdfs:range rdf:resource="http://www.w3.org/2001/XMLSchema#string"/>
  </owl:DatatypeProperty>
  <owl:DatatypeProperty rdf:about="http://example.org/onto/prop/google_backup_dr_backup_plan_delete">
    <rdfs:label>delete</rdfs:label>
    <rdfs:domain rdf:resource="http://example.org/onto/class/google_backup_dr_backup_plan"/>
    <rdfs:range rdf:resource="http://www.w3.org/2001/XMLSchema#string"/>
  </owl:DatatypeProperty>
  <owl:DatatypeProperty rdf:about="http://example.org/onto/prop/google_backup_dr_backup_plan_update">
    <rdfs:label>update</rdfs:label>
    <rdfs:domain rdf:resource="http://example.org/onto/class/google_backup_dr_backup_plan"/>
    <rdfs:range rdf:resource="http://www.w3.org/2001/XMLSchema#string"/>
  </owl:DatatypeProperty>
</rdf:RDF>
