<?xml version="1.0" encoding="UTF-8"?>
<rdf:RDF
  xmlns:rdf="http://www.w3.org/1999/02/22-rdf-syntax-ns#"
  xmlns:rdfs="http://www.w3.org/2000/01/rdf-schema#"
  xmlns:owl="http://www.w3.org/2002/07/owl#"
  xmlns:xsd="http://www.w3.org/2001/XMLSchema#"
  xml:base="http://example.org/onto/">
  <owl:Class rdf:about="http://example.org/onto/class/google_vertex_ai_feature_online_store">
    <rdfs:label>google_vertex_ai_feature_online_store</rdfs:label>
    <rdfs:comment>#
#     ***     AUTO GENERATED CODE    ***    Type: MMv1     ***
#
# ----------------------------------------------------------------------------
#
#     This code is generated by Magic Modules using the following:
#
#     Configuration: https:#github.com/GoogleCloudPlatform/magic-modules/tree/main/mmv1/products/vertexai/FeatureOnlineStore.yaml
#     Template:      https:#github.com/GoogleCloudPlatform/magic-modules/tree/main/mmv1/templates/terraform/resource.html.markdown.tmpl
#
#     DO NOT EDIT this file directly. Any changes made to this file will be
#     overwritten during the next generation cycle.
#
# ----------------------------------------------------------------------------
subcategory: "Vertex AI"
description: |-
  Vertex AI Feature Online Store provides a centralized repository for serving ML features and embedding indexes at low latency.
---</rdfs:comment>
  </owl:Class>
  <owl:DatatypeProperty rdf:about="http://example.org/onto/prop/google_vertex_ai_feature_online_store_create_time">
    <rdfs:label>create_time</rdfs:label>
    <rdfs:comment>The timestamp of when the feature online store was created in RFC3339 UTC "Zulu" format, with nanosecond resolution and up to nine fractional digits.</rdfs:comment>
    <rdfs:domain rdf:resource="http://example.org/onto/class/google_vertex_ai_feature_online_store"/>
    <rdfs:range rdf:resource="http://www.w3.org/2001/XMLSchema#string"/>
  </owl:DatatypeProperty>
  <owl:DatatypeProperty rdf:about="http://example.org/onto/prop/google_vertex_ai_feature_online_store_effective_labels">
    <rdfs:label>effective_labels</rdfs:label>
    <rdfs:comment>All of labels (key/value pairs) present on the resource in GCP, including the labels configured through Terraform, other clients and services.</rdfs:comment>
    <rdfs:domain rdf:resource="http://example.org/onto/class/google_vertex_ai_feature_online_store"/>
    <rdfs:range rdf:resource="http://www.w3.org/2001/XMLSchema#string"/>
  </owl:DatatypeProperty>
  <owl:DatatypeProperty rdf:about="http://example.org/onto/prop/google_vertex_ai_feature_online_store_etag">
    <rdfs:label>etag</rdfs:label>
    <rdfs:comment>Used to perform consistent read-modify-write updates.</rdfs:comment>
    <rdfs:domain rdf:resource="http://example.org/onto/class/google_vertex_ai_feature_online_store"/>
    <rdfs:range rdf:resource="http://www.w3.org/2001/XMLSchema#string"/>
  </owl:DatatypeProperty>
  <owl:DatatypeProperty rdf:about="http://example.org/onto/prop/google_vertex_ai_feature_online_store_force_destroy">
    <rdfs:label>force_destroy</rdfs:label>
    <rdfs:comment>If set to true, any FeatureViews and Features for this FeatureOnlineStore will also be deleted.</rdfs:comment>
    <rdfs:domain rdf:resource="http://example.org/onto/class/google_vertex_ai_feature_online_store"/>
    <rdfs:range rdf:resource="http://www.w3.org/2001/XMLSchema#string"/>
  </owl:DatatypeProperty>
  <owl:DatatypeProperty rdf:about="http://example.org/onto/prop/google_vertex_ai_feature_online_store_id">
    <rdfs:label>id</rdfs:label>
    <rdfs:domain rdf:resource="http://example.org/onto/class/google_vertex_ai_feature_online_store"/>
    <rdfs:range rdf:resource="http://www.w3.org/2001/XMLSchema#string"/>
  </owl:DatatypeProperty>
  <owl:DatatypeProperty rdf:about="http://example.org/onto/prop/google_vertex_ai_feature_online_store_labels">
    <rdfs:label>labels</rdfs:label>
    <rdfs:comment>The labels with user-defined metadata to organize your feature online stores.

**Note**: This field is non-authoritative, and will only manage the labels present in your configuration.
Please refer to the field 'effective_labels' for all of the labels present on the resource.</rdfs:comment>
    <rdfs:domain rdf:resource="http://example.org/onto/class/google_vertex_ai_feature_online_store"/>
    <rdfs:range rdf:resource="http://www.w3.org/2001/XMLSchema#string"/>
  </owl:DatatypeProperty>
  <owl:DatatypeProperty rdf:about="http://example.org/onto/prop/google_vertex_ai_feature_online_store_name">
    <rdfs:label>name</rdfs:label>
    <rdfs:comment>The resource name of the Feature Online Store. This value may be up to 60 characters, and valid characters are [a-z0-9_]. The first character cannot be a number.</rdfs:comment>
    <rdfs:domain rdf:resource="http://example.org/onto/class/google_vertex_ai_feature_online_store"/>
    <rdfs:range rdf:resource="http://www.w3.org/2001/XMLSchema#string"/>
  </owl:DatatypeProperty>
  <owl:DatatypeProperty rdf:about="http://example.org/onto/prop/google_vertex_ai_feature_online_store_project">
    <rdfs:label>project</rdfs:label>
    <rdfs:domain rdf:resource="http://example.org/onto/class/google_vertex_ai_feature_online_store"/>
    <rdfs:range rdf:resource="http://www.w3.org/2001/XMLSchema#string"/>
  </owl:DatatypeProperty>
  <owl:DatatypeProperty rdf:about="http://example.org/onto/prop/google_vertex_ai_feature_online_store_region">
    <rdfs:label>region</rdfs:label>
    <rdfs:comment>The region of feature online store. eg us-central1</rdfs:comment>
    <rdfs:domain rdf:resource="http://example.org/onto/class/google_vertex_ai_feature_online_store"/>
    <rdfs:range rdf:resource="http://www.w3.org/2001/XMLSchema#string"/>
  </owl:DatatypeProperty>
  <owl:DatatypeProperty rdf:about="http://example.org/onto/prop/google_vertex_ai_feature_online_store_state">
    <rdfs:label>state</rdfs:label>
    <rdfs:comment>The state of the Feature Online Store. See the possible states in [this link](https://cloud.google.com/vertex-ai/docs/reference/rest/v1/projects.locations.featureOnlineStores#state).</rdfs:comment>
    <rdfs:domain rdf:resource="http://example.org/onto/class/google_vertex_ai_feature_online_store"/>
    <rdfs:range rdf:resource="http://www.w3.org/2001/XMLSchema#string"/>
  </owl:DatatypeProperty>
  <owl:DatatypeProperty rdf:about="http://example.org/onto/prop/google_vertex_ai_feature_online_store_terraform_labels">
    <rdfs:label>terraform_labels</rdfs:label>
    <rdfs:comment>The combination of labels configured directly on the resource
 and default labels configured on the provider.</rdfs:comment>
    <rdfs:domain rdf:resource="http://example.org/onto/class/google_vertex_ai_feature_online_store"/>
    <rdfs:range rdf:resource="http://www.w3.org/2001/XMLSchema#string"/>
  </owl:DatatypeProperty>
  <owl:DatatypeProperty rdf:about="http://example.org/onto/prop/google_vertex_ai_feature_online_store_update_time">
    <rdfs:label>update_time</rdfs:label>
    <rdfs:comment>The timestamp of when the feature online store was last updated in RFC3339 UTC "Zulu" format, with nanosecond resolution and up to nine fractional digits.</rdfs:comment>
    <rdfs:domain rdf:resource="http://example.org/onto/class/google_vertex_ai_feature_online_store"/>
    <rdfs:range rdf:resource="http://www.w3.org/2001/XMLSchema#string"/>
  </owl:DatatypeProperty>
  <owl:DatatypeProperty rdf:about="http://example.org/onto/prop/google_vertex_ai_feature_online_store_cpu_utilization_target">
    <rdfs:label>cpu_utilization_target</rdfs:label>
    <rdfs:comment>A percentage of the cluster's CPU capacity. Can be from 10% to 80%. When a cluster's CPU utilization exceeds the target that you have set, Bigtable immediately adds nodes to the cluster. When CPU utilization is substantially lower than the target, Bigtable removes nodes. If not set will default to 50%.</rdfs:comment>
    <rdfs:domain rdf:resource="http://example.org/onto/class/google_vertex_ai_feature_online_store"/>
    <rdfs:range rdf:resource="http://www.w3.org/2001/XMLSchema#string"/>
  </owl:DatatypeProperty>
  <owl:DatatypeProperty rdf:about="http://example.org/onto/prop/google_vertex_ai_feature_online_store_max_node_count">
    <rdfs:label>max_node_count</rdfs:label>
    <rdfs:comment>The maximum number of nodes to scale up to. Must be greater than or equal to minNodeCount, and less than or equal to 10 times of 'minNodeCount'.</rdfs:comment>
    <rdfs:domain rdf:resource="http://example.org/onto/class/google_vertex_ai_feature_online_store"/>
    <rdfs:range rdf:resource="http://www.w3.org/2001/XMLSchema#string"/>
  </owl:DatatypeProperty>
  <owl:DatatypeProperty rdf:about="http://example.org/onto/prop/google_vertex_ai_feature_online_store_min_node_count">
    <rdfs:label>min_node_count</rdfs:label>
    <rdfs:comment>The minimum number of nodes to scale down to. Must be greater than or equal to 1.</rdfs:comment>
    <rdfs:domain rdf:resource="http://example.org/onto/class/google_vertex_ai_feature_online_store"/>
    <rdfs:range rdf:resource="http://www.w3.org/2001/XMLSchema#string"/>
  </owl:DatatypeProperty>
  <owl:DatatypeProperty rdf:about="http://example.org/onto/prop/google_vertex_ai_feature_online_store_public_endpoint_domain_name">
    <rdfs:label>public_endpoint_domain_name</rdfs:label>
    <rdfs:comment>Domain name to use for this FeatureOnlineStore</rdfs:comment>
    <rdfs:domain rdf:resource="http://example.org/onto/class/google_vertex_ai_feature_online_store"/>
    <rdfs:range rdf:resource="http://www.w3.org/2001/XMLSchema#string"/>
  </owl:DatatypeProperty>
  <owl:DatatypeProperty rdf:about="http://example.org/onto/prop/google_vertex_ai_feature_online_store_service_attachment">
    <rdfs:label>service_attachment</rdfs:label>
    <rdfs:comment>Name of the service attachment resource. Applicable only if private service connect is enabled and after FeatureViewSync is created.</rdfs:comment>
    <rdfs:domain rdf:resource="http://example.org/onto/class/google_vertex_ai_feature_online_store"/>
    <rdfs:range rdf:resource="http://www.w3.org/2001/XMLSchema#string"/>
  </owl:DatatypeProperty>
  <owl:DatatypeProperty rdf:about="http://example.org/onto/prop/google_vertex_ai_feature_online_store_enable_private_service_connect">
    <rdfs:label>enable_private_service_connect</rdfs:label>
    <rdfs:comment>If set to true, customers will use private service connection to send request. Otherwise, the connection will set to public endpoint.</rdfs:comment>
    <rdfs:domain rdf:resource="http://example.org/onto/class/google_vertex_ai_feature_online_store"/>
    <rdfs:range rdf:resource="http://www.w3.org/2001/XMLSchema#string"/>
  </owl:DatatypeProperty>
  <owl:DatatypeProperty rdf:about="http://example.org/onto/prop/google_vertex_ai_feature_online_store_project_allowlist">
    <rdfs:label>project_allowlist</rdfs:label>
    <rdfs:comment>A list of Projects from which the forwarding rule will target the service attachment.</rdfs:comment>
    <rdfs:domain rdf:resource="http://example.org/onto/class/google_vertex_ai_feature_online_store"/>
    <rdfs:range rdf:resource="http://www.w3.org/2001/XMLSchema#string"/>
  </owl:DatatypeProperty>
  <owl:DatatypeProperty rdf:about="http://example.org/onto/prop/google_vertex_ai_feature_online_store_create">
    <rdfs:label>create</rdfs:label>
    <rdfs:domain rdf:resource="http://example.org/onto/class/google_vertex_ai_feature_online_store"/>
    <rdfs:range rdf:resource="http://www.w3.org/2001/XMLSchema#string"/>
  </owl:DatatypeProperty>
  <owl:DatatypeProperty rdf:about="http://example.org/onto/prop/google_vertex_ai_feature_online_store_delete">
    <rdfs:label>delete</rdfs:label>
    <rdfs:domain rdf:resource="http://example.org/onto/class/google_vertex_ai_feature_online_store"/>
    <rdfs:range rdf:resource="http://www.w3.org/2001/XMLSchema#string"/>
  </owl:DatatypeProperty>
  <owl:DatatypeProperty rdf:about="http://example.org/onto/prop/google_vertex_ai_feature_online_store_update">
    <rdfs:label>update</rdfs:label>
    <rdfs:domain rdf:resource="http://example.org/onto/class/google_vertex_ai_feature_online_store"/>
    <rdfs:range rdf:resource="http://www.w3.org/2001/XMLSchema#string"/>
  </owl:DatatypeProperty>
</rdf:RDF>
