<?xml version="1.0" encoding="UTF-8"?>
<rdf:RDF
  xmlns:rdf="http://www.w3.org/1999/02/22-rdf-syntax-ns#"
  xmlns:rdfs="http://www.w3.org/2000/01/rdf-schema#"
  xmlns:owl="http://www.w3.org/2002/07/owl#"
  xmlns:xsd="http://www.w3.org/2001/XMLSchema#"
  xml:base="http://example.org/onto/">
  <owl:Class rdf:about="http://example.org/onto/class/google_compute_firewall">
    <rdfs:label>google_compute_firewall</rdfs:label>
    <rdfs:comment>#
#     ***     AUTO GENERATED CODE    ***    Type: MMv1     ***
#
# ----------------------------------------------------------------------------
#
#     This code is generated by Magic Modules using the following:
#
#     Configuration: https:#github.com/GoogleCloudPlatform/magic-modules/tree/main/mmv1/products/compute/Firewall.yaml
#     Template:      https:#github.com/GoogleCloudPlatform/magic-modules/tree/main/mmv1/templates/terraform/resource.html.markdown.tmpl
#
#     DO NOT EDIT this file directly. Any changes made to this file will be
#     overwritten during the next generation cycle.
#
# ----------------------------------------------------------------------------
subcategory: "Compute Engine"
description: |-
  Each network has its own firewall controlling access to and from the
  instances.
---</rdfs:comment>
  </owl:Class>
  <owl:DatatypeProperty rdf:about="http://example.org/onto/prop/google_compute_firewall_creation_timestamp">
    <rdfs:label>creation_timestamp</rdfs:label>
    <rdfs:comment>Creation timestamp in RFC3339 text format.</rdfs:comment>
    <rdfs:domain rdf:resource="http://example.org/onto/class/google_compute_firewall"/>
    <rdfs:range rdf:resource="http://www.w3.org/2001/XMLSchema#string"/>
  </owl:DatatypeProperty>
  <owl:DatatypeProperty rdf:about="http://example.org/onto/prop/google_compute_firewall_description">
    <rdfs:label>description</rdfs:label>
    <rdfs:comment>An optional description of this resource. Provide this property when
you create the resource.</rdfs:comment>
    <rdfs:domain rdf:resource="http://example.org/onto/class/google_compute_firewall"/>
    <rdfs:range rdf:resource="http://www.w3.org/2001/XMLSchema#string"/>
  </owl:DatatypeProperty>
  <owl:DatatypeProperty rdf:about="http://example.org/onto/prop/google_compute_firewall_destination_ranges">
    <rdfs:label>destination_ranges</rdfs:label>
    <rdfs:comment>If destination ranges are specified, the firewall will apply only to
traffic that has destination IP address in these ranges. These ranges
must be expressed in CIDR format. IPv4 or IPv6 ranges are supported.</rdfs:comment>
    <rdfs:domain rdf:resource="http://example.org/onto/class/google_compute_firewall"/>
    <rdfs:range rdf:resource="http://www.w3.org/2001/XMLSchema#string"/>
  </owl:DatatypeProperty>
  <owl:DatatypeProperty rdf:about="http://example.org/onto/prop/google_compute_firewall_direction">
    <rdfs:label>direction</rdfs:label>
    <rdfs:comment>Direction of traffic to which this firewall applies; default is
INGRESS. Note: For INGRESS traffic, one of 'source_ranges',
'source_tags' or 'source_service_accounts' is required. Possible values: ["INGRESS", "EGRESS"]</rdfs:comment>
    <rdfs:domain rdf:resource="http://example.org/onto/class/google_compute_firewall"/>
    <rdfs:range rdf:resource="http://www.w3.org/2001/XMLSchema#string"/>
  </owl:DatatypeProperty>
  <owl:DatatypeProperty rdf:about="http://example.org/onto/prop/google_compute_firewall_disabled">
    <rdfs:label>disabled</rdfs:label>
    <rdfs:comment>Denotes whether the firewall rule is disabled, i.e not applied to the
network it is associated with. When set to true, the firewall rule is
not enforced and the network behaves as if it did not exist. If this
is unspecified, the firewall rule will be enabled.</rdfs:comment>
    <rdfs:domain rdf:resource="http://example.org/onto/class/google_compute_firewall"/>
    <rdfs:range rdf:resource="http://www.w3.org/2001/XMLSchema#string"/>
  </owl:DatatypeProperty>
  <owl:DatatypeProperty rdf:about="http://example.org/onto/prop/google_compute_firewall_enable_logging">
    <rdfs:label>enable_logging</rdfs:label>
    <rdfs:comment>This field denotes whether to enable logging for a particular firewall rule. If logging is enabled, logs will be exported to Stackdriver.</rdfs:comment>
    <rdfs:domain rdf:resource="http://example.org/onto/class/google_compute_firewall"/>
    <rdfs:range rdf:resource="http://www.w3.org/2001/XMLSchema#string"/>
  </owl:DatatypeProperty>
  <owl:DatatypeProperty rdf:about="http://example.org/onto/prop/google_compute_firewall_id">
    <rdfs:label>id</rdfs:label>
    <rdfs:domain rdf:resource="http://example.org/onto/class/google_compute_firewall"/>
    <rdfs:range rdf:resource="http://www.w3.org/2001/XMLSchema#string"/>
  </owl:DatatypeProperty>
  <owl:DatatypeProperty rdf:about="http://example.org/onto/prop/google_compute_firewall_name">
    <rdfs:label>name</rdfs:label>
    <rdfs:comment>Name of the resource. Provided by the client when the resource is
created. The name must be 1-63 characters long, and comply with
RFC1035. Specifically, the name must be 1-63 characters long and match
the regular expression '[a-z]([-a-z0-9]*[a-z0-9])?' which means the
first character must be a lowercase letter, and all following
characters must be a dash, lowercase letter, or digit, except the last
character, which cannot be a dash.</rdfs:comment>
    <rdfs:domain rdf:resource="http://example.org/onto/class/google_compute_firewall"/>
    <rdfs:range rdf:resource="http://www.w3.org/2001/XMLSchema#string"/>
  </owl:DatatypeProperty>
  <owl:DatatypeProperty rdf:about="http://example.org/onto/prop/google_compute_firewall_network">
    <rdfs:label>network</rdfs:label>
    <rdfs:comment>The name or self_link of the network to attach this firewall to.</rdfs:comment>
    <rdfs:domain rdf:resource="http://example.org/onto/class/google_compute_firewall"/>
    <rdfs:range rdf:resource="http://www.w3.org/2001/XMLSchema#string"/>
  </owl:DatatypeProperty>
  <owl:DatatypeProperty rdf:about="http://example.org/onto/prop/google_compute_firewall_priority">
    <rdfs:label>priority</rdfs:label>
    <rdfs:comment>Priority for this rule. This is an integer between 0 and 65535, both
inclusive. When not specified, the value assumed is 1000. Relative
priorities determine precedence of conflicting rules. Lower value of
priority implies higher precedence (eg, a rule with priority 0 has
higher precedence than a rule with priority 1). DENY rules take
precedence over ALLOW rules having equal priority.</rdfs:comment>
    <rdfs:domain rdf:resource="http://example.org/onto/class/google_compute_firewall"/>
    <rdfs:range rdf:resource="http://www.w3.org/2001/XMLSchema#string"/>
  </owl:DatatypeProperty>
  <owl:DatatypeProperty rdf:about="http://example.org/onto/prop/google_compute_firewall_project">
    <rdfs:label>project</rdfs:label>
    <rdfs:domain rdf:resource="http://example.org/onto/class/google_compute_firewall"/>
    <rdfs:range rdf:resource="http://www.w3.org/2001/XMLSchema#string"/>
  </owl:DatatypeProperty>
  <owl:DatatypeProperty rdf:about="http://example.org/onto/prop/google_compute_firewall_self_link">
    <rdfs:label>self_link</rdfs:label>
    <rdfs:domain rdf:resource="http://example.org/onto/class/google_compute_firewall"/>
    <rdfs:range rdf:resource="http://www.w3.org/2001/XMLSchema#string"/>
  </owl:DatatypeProperty>
  <owl:DatatypeProperty rdf:about="http://example.org/onto/prop/google_compute_firewall_source_ranges">
    <rdfs:label>source_ranges</rdfs:label>
    <rdfs:comment>If source ranges are specified, the firewall will apply only to
traffic that has source IP address in these ranges. These ranges must
be expressed in CIDR format. One or both of sourceRanges and
sourceTags may be set. If both properties are set, the firewall will
apply to traffic that has source IP address within sourceRanges OR the
source IP that belongs to a tag listed in the sourceTags property. The
connection does not need to match both properties for the firewall to
apply. IPv4 or IPv6 ranges are supported. For INGRESS traffic, one of
'source_ranges', 'source_tags' or 'source_service_accounts' is required.</rdfs:comment>
    <rdfs:domain rdf:resource="http://example.org/onto/class/google_compute_firewall"/>
    <rdfs:range rdf:resource="http://www.w3.org/2001/XMLSchema#string"/>
  </owl:DatatypeProperty>
  <owl:DatatypeProperty rdf:about="http://example.org/onto/prop/google_compute_firewall_source_service_accounts">
    <rdfs:label>source_service_accounts</rdfs:label>
    <rdfs:comment>If source service accounts are specified, the firewall will apply only
to traffic originating from an instance with a service account in this
list. Source service accounts cannot be used to control traffic to an
instance's external IP address because service accounts are associated
with an instance, not an IP address. sourceRanges can be set at the
same time as sourceServiceAccounts. If both are set, the firewall will
apply to traffic that has source IP address within sourceRanges OR the
source IP belongs to an instance with service account listed in
sourceServiceAccount. The connection does not need to match both
properties for the firewall to apply. sourceServiceAccounts cannot be
used at the same time as sourceTags or targetTags. For INGRESS traffic,
one of 'source_ranges', 'source_tags' or 'source_service_accounts' is required.</rdfs:comment>
    <rdfs:domain rdf:resource="http://example.org/onto/class/google_compute_firewall"/>
    <rdfs:range rdf:resource="http://www.w3.org/2001/XMLSchema#string"/>
  </owl:DatatypeProperty>
  <owl:DatatypeProperty rdf:about="http://example.org/onto/prop/google_compute_firewall_source_tags">
    <rdfs:label>source_tags</rdfs:label>
    <rdfs:comment>If source tags are specified, the firewall will apply only to traffic
with source IP that belongs to a tag listed in source tags. Source
tags cannot be used to control traffic to an instance's external IP
address. Because tags are associated with an instance, not an IP
address. One or both of sourceRanges and sourceTags may be set. If
both properties are set, the firewall will apply to traffic that has
source IP address within sourceRanges OR the source IP that belongs to
a tag listed in the sourceTags property. The connection does not need
to match both properties for the firewall to apply. For INGRESS traffic,
one of 'source_ranges', 'source_tags' or 'source_service_accounts' is required.</rdfs:comment>
    <rdfs:domain rdf:resource="http://example.org/onto/class/google_compute_firewall"/>
    <rdfs:range rdf:resource="http://www.w3.org/2001/XMLSchema#string"/>
  </owl:DatatypeProperty>
  <owl:DatatypeProperty rdf:about="http://example.org/onto/prop/google_compute_firewall_target_service_accounts">
    <rdfs:label>target_service_accounts</rdfs:label>
    <rdfs:comment>A list of service accounts indicating sets of instances located in the
network that may make network connections as specified in allowed[].
targetServiceAccounts cannot be used at the same time as targetTags or
sourceTags. If neither targetServiceAccounts nor targetTags are
specified, the firewall rule applies to all instances on the specified
network.</rdfs:comment>
    <rdfs:domain rdf:resource="http://example.org/onto/class/google_compute_firewall"/>
    <rdfs:range rdf:resource="http://www.w3.org/2001/XMLSchema#string"/>
  </owl:DatatypeProperty>
  <owl:DatatypeProperty rdf:about="http://example.org/onto/prop/google_compute_firewall_target_tags">
    <rdfs:label>target_tags</rdfs:label>
    <rdfs:comment>A list of instance tags indicating sets of instances located in the
network that may make network connections as specified in allowed[].
If no targetTags are specified, the firewall rule applies to all
instances on the specified network.</rdfs:comment>
    <rdfs:domain rdf:resource="http://example.org/onto/class/google_compute_firewall"/>
    <rdfs:range rdf:resource="http://www.w3.org/2001/XMLSchema#string"/>
  </owl:DatatypeProperty>
  <owl:DatatypeProperty rdf:about="http://example.org/onto/prop/google_compute_firewall_ports">
    <rdfs:label>ports</rdfs:label>
    <rdfs:comment>An optional list of ports to which this rule applies. This field
is only applicable for UDP or TCP protocol. Each entry must be
either an integer or a range. If not specified, this rule
applies to connections through any port.

Example inputs include: [22], [80, 443], and
["12345-12349"].</rdfs:comment>
    <rdfs:domain rdf:resource="http://example.org/onto/class/google_compute_firewall"/>
    <rdfs:range rdf:resource="http://www.w3.org/2001/XMLSchema#string"/>
  </owl:DatatypeProperty>
  <owl:DatatypeProperty rdf:about="http://example.org/onto/prop/google_compute_firewall_protocol">
    <rdfs:label>protocol</rdfs:label>
    <rdfs:comment>The IP protocol to which this rule applies. The protocol type is
required when creating a firewall rule. This value can either be
one of the following well known protocol strings (tcp, udp,
icmp, esp, ah, sctp, ipip, all), or the IP protocol number.</rdfs:comment>
    <rdfs:domain rdf:resource="http://example.org/onto/class/google_compute_firewall"/>
    <rdfs:range rdf:resource="http://www.w3.org/2001/XMLSchema#string"/>
  </owl:DatatypeProperty>
  <owl:DatatypeProperty rdf:about="http://example.org/onto/prop/google_compute_firewall_ports">
    <rdfs:label>ports</rdfs:label>
    <rdfs:comment>An optional list of ports to which this rule applies. This field
is only applicable for UDP or TCP protocol. Each entry must be
either an integer or a range. If not specified, this rule
applies to connections through any port.

Example inputs include: [22], [80, 443], and
["12345-12349"].</rdfs:comment>
    <rdfs:domain rdf:resource="http://example.org/onto/class/google_compute_firewall"/>
    <rdfs:range rdf:resource="http://www.w3.org/2001/XMLSchema#string"/>
  </owl:DatatypeProperty>
  <owl:DatatypeProperty rdf:about="http://example.org/onto/prop/google_compute_firewall_protocol">
    <rdfs:label>protocol</rdfs:label>
    <rdfs:comment>The IP protocol to which this rule applies. The protocol type is
required when creating a firewall rule. This value can either be
one of the following well known protocol strings (tcp, udp,
icmp, esp, ah, sctp, ipip, all), or the IP protocol number.</rdfs:comment>
    <rdfs:domain rdf:resource="http://example.org/onto/class/google_compute_firewall"/>
    <rdfs:range rdf:resource="http://www.w3.org/2001/XMLSchema#string"/>
  </owl:DatatypeProperty>
  <owl:DatatypeProperty rdf:about="http://example.org/onto/prop/google_compute_firewall_metadata">
    <rdfs:label>metadata</rdfs:label>
    <rdfs:comment>This field denotes whether to include or exclude metadata for firewall logs. Possible values: ["EXCLUDE_ALL_METADATA", "INCLUDE_ALL_METADATA"]</rdfs:comment>
    <rdfs:domain rdf:resource="http://example.org/onto/class/google_compute_firewall"/>
    <rdfs:range rdf:resource="http://www.w3.org/2001/XMLSchema#string"/>
  </owl:DatatypeProperty>
  <owl:DatatypeProperty rdf:about="http://example.org/onto/prop/google_compute_firewall_resource_manager_tags">
    <rdfs:label>resource_manager_tags</rdfs:label>
    <rdfs:comment>Resource manager tags to be bound to the firewall. Tag keys and values have the
same definition as resource manager tags. Keys must be in the format tagKeys/{tag_key_id},
and values are in the format tagValues/456. The field is ignored when empty.
The field is immutable and causes resource replacement when mutated. This field is only
set at create time and modifying this field after creation will trigger recreation.
To apply tags to an existing resource, see the google_tags_tag_binding resource.</rdfs:comment>
    <rdfs:domain rdf:resource="http://example.org/onto/class/google_compute_firewall"/>
    <rdfs:range rdf:resource="http://www.w3.org/2001/XMLSchema#string"/>
  </owl:DatatypeProperty>
  <owl:DatatypeProperty rdf:about="http://example.org/onto/prop/google_compute_firewall_create">
    <rdfs:label>create</rdfs:label>
    <rdfs:domain rdf:resource="http://example.org/onto/class/google_compute_firewall"/>
    <rdfs:range rdf:resource="http://www.w3.org/2001/XMLSchema#string"/>
  </owl:DatatypeProperty>
  <owl:DatatypeProperty rdf:about="http://example.org/onto/prop/google_compute_firewall_delete">
    <rdfs:label>delete</rdfs:label>
    <rdfs:domain rdf:resource="http://example.org/onto/class/google_compute_firewall"/>
    <rdfs:range rdf:resource="http://www.w3.org/2001/XMLSchema#string"/>
  </owl:DatatypeProperty>
  <owl:DatatypeProperty rdf:about="http://example.org/onto/prop/google_compute_firewall_update">
    <rdfs:label>update</rdfs:label>
    <rdfs:domain rdf:resource="http://example.org/onto/class/google_compute_firewall"/>
    <rdfs:range rdf:resource="http://www.w3.org/2001/XMLSchema#string"/>
  </owl:DatatypeProperty>
</rdf:RDF>
