<?xml version="1.0" encoding="UTF-8"?>
<rdf:RDF
  xmlns:rdf="http://www.w3.org/1999/02/22-rdf-syntax-ns#"
  xmlns:rdfs="http://www.w3.org/2000/01/rdf-schema#"
  xmlns:owl="http://www.w3.org/2002/07/owl#"
  xmlns:xsd="http://www.w3.org/2001/XMLSchema#"
  xml:base="http://example.org/onto/">
  <owl:Class rdf:about="http://example.org/onto/class/google_alloydb_backup">
    <rdfs:label>google_alloydb_backup</rdfs:label>
    <rdfs:comment>#
#     ***     AUTO GENERATED CODE    ***    Type: MMv1     ***
#
# ----------------------------------------------------------------------------
#
#     This code is generated by Magic Modules using the following:
#
#     Configuration: https:#github.com/GoogleCloudPlatform/magic-modules/tree/main/mmv1/products/alloydb/Backup.yaml
#     Template:      https:#github.com/GoogleCloudPlatform/magic-modules/tree/main/mmv1/templates/terraform/resource.html.markdown.tmpl
#
#     DO NOT EDIT this file directly. Any changes made to this file will be
#     overwritten during the next generation cycle.
#
# ----------------------------------------------------------------------------
subcategory: "AlloyDB"
description: |-
  An AlloyDB Backup.
---</rdfs:comment>
  </owl:Class>
  <owl:DatatypeProperty rdf:about="http://example.org/onto/prop/google_alloydb_backup_annotations">
    <rdfs:label>annotations</rdfs:label>
    <rdfs:comment>Annotations to allow client tools to store small amount of arbitrary data. This is distinct from labels. https://google.aip.dev/128
An object containing a list of "key": value pairs. Example: { "name": "wrench", "mass": "1.3kg", "count": "3" }.


**Note**: This field is non-authoritative, and will only manage the annotations present in your configuration.
Please refer to the field 'effective_annotations' for all of the annotations present on the resource.</rdfs:comment>
    <rdfs:domain rdf:resource="http://example.org/onto/class/google_alloydb_backup"/>
    <rdfs:range rdf:resource="http://www.w3.org/2001/XMLSchema#string"/>
  </owl:DatatypeProperty>
  <owl:DatatypeProperty rdf:about="http://example.org/onto/prop/google_alloydb_backup_backup_id">
    <rdfs:label>backup_id</rdfs:label>
    <rdfs:comment>The ID of the alloydb backup.</rdfs:comment>
    <rdfs:domain rdf:resource="http://example.org/onto/class/google_alloydb_backup"/>
    <rdfs:range rdf:resource="http://www.w3.org/2001/XMLSchema#string"/>
  </owl:DatatypeProperty>
  <owl:DatatypeProperty rdf:about="http://example.org/onto/prop/google_alloydb_backup_cluster_name">
    <rdfs:label>cluster_name</rdfs:label>
    <rdfs:comment>The full resource name of the backup source cluster (e.g., projects/{project}/locations/{location}/clusters/{clusterId}).</rdfs:comment>
    <rdfs:domain rdf:resource="http://example.org/onto/class/google_alloydb_backup"/>
    <rdfs:range rdf:resource="http://www.w3.org/2001/XMLSchema#string"/>
  </owl:DatatypeProperty>
  <owl:DatatypeProperty rdf:about="http://example.org/onto/prop/google_alloydb_backup_cluster_uid">
    <rdfs:label>cluster_uid</rdfs:label>
    <rdfs:comment>Output only. The system-generated UID of the cluster which was used to create this resource.</rdfs:comment>
    <rdfs:domain rdf:resource="http://example.org/onto/class/google_alloydb_backup"/>
    <rdfs:range rdf:resource="http://www.w3.org/2001/XMLSchema#string"/>
  </owl:DatatypeProperty>
  <owl:DatatypeProperty rdf:about="http://example.org/onto/prop/google_alloydb_backup_create_time">
    <rdfs:label>create_time</rdfs:label>
    <rdfs:comment>Output only. Create time stamp. A timestamp in RFC3339 UTC "Zulu" format, with nanosecond resolution and up to nine fractional digits.
Examples: "2014-10-02T15:01:23Z" and "2014-10-02T15:01:23.045123456Z".</rdfs:comment>
    <rdfs:domain rdf:resource="http://example.org/onto/class/google_alloydb_backup"/>
    <rdfs:range rdf:resource="http://www.w3.org/2001/XMLSchema#string"/>
  </owl:DatatypeProperty>
  <owl:DatatypeProperty rdf:about="http://example.org/onto/prop/google_alloydb_backup_delete_time">
    <rdfs:label>delete_time</rdfs:label>
    <rdfs:comment>Output only. Delete time stamp. A timestamp in RFC3339 UTC "Zulu" format, with nanosecond resolution and up to nine fractional digits.
Examples: "2014-10-02T15:01:23Z" and "2014-10-02T15:01:23.045123456Z".</rdfs:comment>
    <rdfs:domain rdf:resource="http://example.org/onto/class/google_alloydb_backup"/>
    <rdfs:range rdf:resource="http://www.w3.org/2001/XMLSchema#string"/>
  </owl:DatatypeProperty>
  <owl:DatatypeProperty rdf:about="http://example.org/onto/prop/google_alloydb_backup_description">
    <rdfs:label>description</rdfs:label>
    <rdfs:comment>User-provided description of the backup.</rdfs:comment>
    <rdfs:domain rdf:resource="http://example.org/onto/class/google_alloydb_backup"/>
    <rdfs:range rdf:resource="http://www.w3.org/2001/XMLSchema#string"/>
  </owl:DatatypeProperty>
  <owl:DatatypeProperty rdf:about="http://example.org/onto/prop/google_alloydb_backup_display_name">
    <rdfs:label>display_name</rdfs:label>
    <rdfs:comment>User-settable and human-readable display name for the Backup.</rdfs:comment>
    <rdfs:domain rdf:resource="http://example.org/onto/class/google_alloydb_backup"/>
    <rdfs:range rdf:resource="http://www.w3.org/2001/XMLSchema#string"/>
  </owl:DatatypeProperty>
  <owl:DatatypeProperty rdf:about="http://example.org/onto/prop/google_alloydb_backup_effective_annotations">
    <rdfs:label>effective_annotations</rdfs:label>
    <rdfs:comment>All of annotations (key/value pairs) present on the resource in GCP, including the annotations configured through Terraform, other clients and services.</rdfs:comment>
    <rdfs:domain rdf:resource="http://example.org/onto/class/google_alloydb_backup"/>
    <rdfs:range rdf:resource="http://www.w3.org/2001/XMLSchema#string"/>
  </owl:DatatypeProperty>
  <owl:DatatypeProperty rdf:about="http://example.org/onto/prop/google_alloydb_backup_effective_labels">
    <rdfs:label>effective_labels</rdfs:label>
    <rdfs:comment>All of labels (key/value pairs) present on the resource in GCP, including the labels configured through Terraform, other clients and services.</rdfs:comment>
    <rdfs:domain rdf:resource="http://example.org/onto/class/google_alloydb_backup"/>
    <rdfs:range rdf:resource="http://www.w3.org/2001/XMLSchema#string"/>
  </owl:DatatypeProperty>
  <owl:DatatypeProperty rdf:about="http://example.org/onto/prop/google_alloydb_backup_encryption_info">
    <rdfs:label>encryption_info</rdfs:label>
    <rdfs:comment>EncryptionInfo describes the encryption information of a cluster or a backup.</rdfs:comment>
    <rdfs:domain rdf:resource="http://example.org/onto/class/google_alloydb_backup"/>
    <rdfs:range rdf:resource="http://www.w3.org/2001/XMLSchema#string"/>
  </owl:DatatypeProperty>
  <owl:DatatypeProperty rdf:about="http://example.org/onto/prop/google_alloydb_backup_etag">
    <rdfs:label>etag</rdfs:label>
    <rdfs:comment>For Resource freshness validation (https://google.aip.dev/154)</rdfs:comment>
    <rdfs:domain rdf:resource="http://example.org/onto/class/google_alloydb_backup"/>
    <rdfs:range rdf:resource="http://www.w3.org/2001/XMLSchema#string"/>
  </owl:DatatypeProperty>
  <owl:DatatypeProperty rdf:about="http://example.org/onto/prop/google_alloydb_backup_expiry_quantity">
    <rdfs:label>expiry_quantity</rdfs:label>
    <rdfs:comment>Output only. The QuantityBasedExpiry of the backup, specified by the backup's retention policy.
Once the expiry quantity is over retention, the backup is eligible to be garbage collected.</rdfs:comment>
    <rdfs:domain rdf:resource="http://example.org/onto/class/google_alloydb_backup"/>
    <rdfs:range rdf:resource="http://www.w3.org/2001/XMLSchema#string"/>
  </owl:DatatypeProperty>
  <owl:DatatypeProperty rdf:about="http://example.org/onto/prop/google_alloydb_backup_expiry_time">
    <rdfs:label>expiry_time</rdfs:label>
    <rdfs:comment>Output only. The time at which after the backup is eligible to be garbage collected.
It is the duration specified by the backup's retention policy, added to the backup's createTime.</rdfs:comment>
    <rdfs:domain rdf:resource="http://example.org/onto/class/google_alloydb_backup"/>
    <rdfs:range rdf:resource="http://www.w3.org/2001/XMLSchema#string"/>
  </owl:DatatypeProperty>
  <owl:DatatypeProperty rdf:about="http://example.org/onto/prop/google_alloydb_backup_id">
    <rdfs:label>id</rdfs:label>
    <rdfs:domain rdf:resource="http://example.org/onto/class/google_alloydb_backup"/>
    <rdfs:range rdf:resource="http://www.w3.org/2001/XMLSchema#string"/>
  </owl:DatatypeProperty>
  <owl:DatatypeProperty rdf:about="http://example.org/onto/prop/google_alloydb_backup_labels">
    <rdfs:label>labels</rdfs:label>
    <rdfs:comment>User-defined labels for the alloydb backup. An object containing a list of "key": value pairs. Example: { "name": "wrench", "mass": "1.3kg", "count": "3" }.


**Note**: This field is non-authoritative, and will only manage the labels present in your configuration.
Please refer to the field 'effective_labels' for all of the labels present on the resource.</rdfs:comment>
    <rdfs:domain rdf:resource="http://example.org/onto/class/google_alloydb_backup"/>
    <rdfs:range rdf:resource="http://www.w3.org/2001/XMLSchema#string"/>
  </owl:DatatypeProperty>
  <owl:DatatypeProperty rdf:about="http://example.org/onto/prop/google_alloydb_backup_location">
    <rdfs:label>location</rdfs:label>
    <rdfs:comment>The location where the alloydb backup should reside.</rdfs:comment>
    <rdfs:domain rdf:resource="http://example.org/onto/class/google_alloydb_backup"/>
    <rdfs:range rdf:resource="http://www.w3.org/2001/XMLSchema#string"/>
  </owl:DatatypeProperty>
  <owl:DatatypeProperty rdf:about="http://example.org/onto/prop/google_alloydb_backup_name">
    <rdfs:label>name</rdfs:label>
    <rdfs:comment>Output only. The name of the backup resource with the format: * projects/{project}/locations/{region}/backups/{backupId}</rdfs:comment>
    <rdfs:domain rdf:resource="http://example.org/onto/class/google_alloydb_backup"/>
    <rdfs:range rdf:resource="http://www.w3.org/2001/XMLSchema#string"/>
  </owl:DatatypeProperty>
  <owl:DatatypeProperty rdf:about="http://example.org/onto/prop/google_alloydb_backup_project">
    <rdfs:label>project</rdfs:label>
    <rdfs:domain rdf:resource="http://example.org/onto/class/google_alloydb_backup"/>
    <rdfs:range rdf:resource="http://www.w3.org/2001/XMLSchema#string"/>
  </owl:DatatypeProperty>
  <owl:DatatypeProperty rdf:about="http://example.org/onto/prop/google_alloydb_backup_reconciling">
    <rdfs:label>reconciling</rdfs:label>
    <rdfs:comment>Output only. Reconciling (https://google.aip.dev/128#reconciliation), if true, indicates that the service is actively updating the resource.
This can happen due to user-triggered updates or system actions like failover or maintenance.</rdfs:comment>
    <rdfs:domain rdf:resource="http://example.org/onto/class/google_alloydb_backup"/>
    <rdfs:range rdf:resource="http://www.w3.org/2001/XMLSchema#string"/>
  </owl:DatatypeProperty>
  <owl:DatatypeProperty rdf:about="http://example.org/onto/prop/google_alloydb_backup_size_bytes">
    <rdfs:label>size_bytes</rdfs:label>
    <rdfs:comment>Output only. The size of the backup in bytes.</rdfs:comment>
    <rdfs:domain rdf:resource="http://example.org/onto/class/google_alloydb_backup"/>
    <rdfs:range rdf:resource="http://www.w3.org/2001/XMLSchema#string"/>
  </owl:DatatypeProperty>
  <owl:DatatypeProperty rdf:about="http://example.org/onto/prop/google_alloydb_backup_state">
    <rdfs:label>state</rdfs:label>
    <rdfs:comment>Output only. The current state of the backup.</rdfs:comment>
    <rdfs:domain rdf:resource="http://example.org/onto/class/google_alloydb_backup"/>
    <rdfs:range rdf:resource="http://www.w3.org/2001/XMLSchema#string"/>
  </owl:DatatypeProperty>
  <owl:DatatypeProperty rdf:about="http://example.org/onto/prop/google_alloydb_backup_terraform_labels">
    <rdfs:label>terraform_labels</rdfs:label>
    <rdfs:comment>The combination of labels configured directly on the resource
 and default labels configured on the provider.</rdfs:comment>
    <rdfs:domain rdf:resource="http://example.org/onto/class/google_alloydb_backup"/>
    <rdfs:range rdf:resource="http://www.w3.org/2001/XMLSchema#string"/>
  </owl:DatatypeProperty>
  <owl:DatatypeProperty rdf:about="http://example.org/onto/prop/google_alloydb_backup_type">
    <rdfs:label>type</rdfs:label>
    <rdfs:comment>The backup type, which suggests the trigger for the backup. Possible values: ["TYPE_UNSPECIFIED", "ON_DEMAND", "AUTOMATED", "CONTINUOUS"]</rdfs:comment>
    <rdfs:domain rdf:resource="http://example.org/onto/class/google_alloydb_backup"/>
    <rdfs:range rdf:resource="http://www.w3.org/2001/XMLSchema#string"/>
  </owl:DatatypeProperty>
  <owl:DatatypeProperty rdf:about="http://example.org/onto/prop/google_alloydb_backup_uid">
    <rdfs:label>uid</rdfs:label>
    <rdfs:comment>Output only. The system-generated UID of the resource. The UID is assigned when the resource is created, and it is retained until it is deleted.</rdfs:comment>
    <rdfs:domain rdf:resource="http://example.org/onto/class/google_alloydb_backup"/>
    <rdfs:range rdf:resource="http://www.w3.org/2001/XMLSchema#string"/>
  </owl:DatatypeProperty>
  <owl:DatatypeProperty rdf:about="http://example.org/onto/prop/google_alloydb_backup_update_time">
    <rdfs:label>update_time</rdfs:label>
    <rdfs:comment>Output only. Update time stamp. A timestamp in RFC3339 UTC "Zulu" format, with nanosecond resolution and up to nine fractional digits.
Examples: "2014-10-02T15:01:23Z" and "2014-10-02T15:01:23.045123456Z".</rdfs:comment>
    <rdfs:domain rdf:resource="http://example.org/onto/class/google_alloydb_backup"/>
    <rdfs:range rdf:resource="http://www.w3.org/2001/XMLSchema#string"/>
  </owl:DatatypeProperty>
  <owl:DatatypeProperty rdf:about="http://example.org/onto/prop/google_alloydb_backup_kms_key_name">
    <rdfs:label>kms_key_name</rdfs:label>
    <rdfs:comment>The fully-qualified resource name of the KMS key. Each Cloud KMS key is regionalized and has the following format: projects/[PROJECT]/locations/[REGION]/keyRings/[RING]/cryptoKeys/[KEY_NAME].</rdfs:comment>
    <rdfs:domain rdf:resource="http://example.org/onto/class/google_alloydb_backup"/>
    <rdfs:range rdf:resource="http://www.w3.org/2001/XMLSchema#string"/>
  </owl:DatatypeProperty>
  <owl:DatatypeProperty rdf:about="http://example.org/onto/prop/google_alloydb_backup_create">
    <rdfs:label>create</rdfs:label>
    <rdfs:domain rdf:resource="http://example.org/onto/class/google_alloydb_backup"/>
    <rdfs:range rdf:resource="http://www.w3.org/2001/XMLSchema#string"/>
  </owl:DatatypeProperty>
  <owl:DatatypeProperty rdf:about="http://example.org/onto/prop/google_alloydb_backup_delete">
    <rdfs:label>delete</rdfs:label>
    <rdfs:domain rdf:resource="http://example.org/onto/class/google_alloydb_backup"/>
    <rdfs:range rdf:resource="http://www.w3.org/2001/XMLSchema#string"/>
  </owl:DatatypeProperty>
  <owl:DatatypeProperty rdf:about="http://example.org/onto/prop/google_alloydb_backup_update">
    <rdfs:label>update</rdfs:label>
    <rdfs:domain rdf:resource="http://example.org/onto/class/google_alloydb_backup"/>
    <rdfs:range rdf:resource="http://www.w3.org/2001/XMLSchema#string"/>
  </owl:DatatypeProperty>
</rdf:RDF>
