<?xml version="1.0" encoding="UTF-8"?>
<rdf:RDF
  xmlns:rdf="http://www.w3.org/1999/02/22-rdf-syntax-ns#"
  xmlns:rdfs="http://www.w3.org/2000/01/rdf-schema#"
  xmlns:owl="http://www.w3.org/2002/07/owl#"
  xmlns:xsd="http://www.w3.org/2001/XMLSchema#"
  xml:base="http://example.org/onto/">
  <owl:Class rdf:about="http://example.org/onto/class/google_database_migration_service_migration_job">
    <rdfs:label>google_database_migration_service_migration_job</rdfs:label>
    <rdfs:comment>#
#     ***     AUTO GENERATED CODE    ***    Type: MMv1     ***
#
# ----------------------------------------------------------------------------
#
#     This code is generated by Magic Modules using the following:
#
#     Configuration: https:#github.com/GoogleCloudPlatform/magic-modules/tree/main/mmv1/products/databasemigrationservice/MigrationJob.yaml
#     Template:      https:#github.com/GoogleCloudPlatform/magic-modules/tree/main/mmv1/templates/terraform/resource.html.markdown.tmpl
#
#     DO NOT EDIT this file directly. Any changes made to this file will be
#     overwritten during the next generation cycle.
#
# ----------------------------------------------------------------------------
subcategory: "DatabaseMigrationService"
description: |-
  A migration job definition.
---</rdfs:comment>
  </owl:Class>
  <owl:DatatypeProperty rdf:about="http://example.org/onto/prop/google_database_migration_service_migration_job_create_time">
    <rdfs:label>create_time</rdfs:label>
    <rdfs:comment>Output only. The timestamp when the resource was created. A timestamp in RFC3339 UTC 'Zulu' format, accurate to nanoseconds. Example: '2014-10-02T15:01:23.045123456Z'.</rdfs:comment>
    <rdfs:domain rdf:resource="http://example.org/onto/class/google_database_migration_service_migration_job"/>
    <rdfs:range rdf:resource="http://www.w3.org/2001/XMLSchema#string"/>
  </owl:DatatypeProperty>
  <owl:DatatypeProperty rdf:about="http://example.org/onto/prop/google_database_migration_service_migration_job_destination">
    <rdfs:label>destination</rdfs:label>
    <rdfs:comment>The name of the destination connection profile resource in the form of projects/{project}/locations/{location}/connectionProfiles/{destinationConnectionProfile}.</rdfs:comment>
    <rdfs:domain rdf:resource="http://example.org/onto/class/google_database_migration_service_migration_job"/>
    <rdfs:range rdf:resource="http://www.w3.org/2001/XMLSchema#string"/>
  </owl:DatatypeProperty>
  <owl:DatatypeProperty rdf:about="http://example.org/onto/prop/google_database_migration_service_migration_job_display_name">
    <rdfs:label>display_name</rdfs:label>
    <rdfs:comment>The migration job display name.</rdfs:comment>
    <rdfs:domain rdf:resource="http://example.org/onto/class/google_database_migration_service_migration_job"/>
    <rdfs:range rdf:resource="http://www.w3.org/2001/XMLSchema#string"/>
  </owl:DatatypeProperty>
  <owl:DatatypeProperty rdf:about="http://example.org/onto/prop/google_database_migration_service_migration_job_dump_path">
    <rdfs:label>dump_path</rdfs:label>
    <rdfs:comment>The path to the dump file in Google Cloud Storage,
in the format: (gs://[BUCKET_NAME]/[OBJECT_NAME]).
This field and the "dump_flags" field are mutually exclusive.</rdfs:comment>
    <rdfs:domain rdf:resource="http://example.org/onto/class/google_database_migration_service_migration_job"/>
    <rdfs:range rdf:resource="http://www.w3.org/2001/XMLSchema#string"/>
  </owl:DatatypeProperty>
  <owl:DatatypeProperty rdf:about="http://example.org/onto/prop/google_database_migration_service_migration_job_dump_type">
    <rdfs:label>dump_type</rdfs:label>
    <rdfs:comment>The type of the data dump. Supported for MySQL to CloudSQL for MySQL
migrations only. Possible values: ["LOGICAL", "PHYSICAL"]</rdfs:comment>
    <rdfs:domain rdf:resource="http://example.org/onto/class/google_database_migration_service_migration_job"/>
    <rdfs:range rdf:resource="http://www.w3.org/2001/XMLSchema#string"/>
  </owl:DatatypeProperty>
  <owl:DatatypeProperty rdf:about="http://example.org/onto/prop/google_database_migration_service_migration_job_effective_labels">
    <rdfs:label>effective_labels</rdfs:label>
    <rdfs:comment>All of labels (key/value pairs) present on the resource in GCP, including the labels configured through Terraform, other clients and services.</rdfs:comment>
    <rdfs:domain rdf:resource="http://example.org/onto/class/google_database_migration_service_migration_job"/>
    <rdfs:range rdf:resource="http://www.w3.org/2001/XMLSchema#string"/>
  </owl:DatatypeProperty>
  <owl:DatatypeProperty rdf:about="http://example.org/onto/prop/google_database_migration_service_migration_job_error">
    <rdfs:label>error</rdfs:label>
    <rdfs:comment>Output only. The error details in case of state FAILED.</rdfs:comment>
    <rdfs:domain rdf:resource="http://example.org/onto/class/google_database_migration_service_migration_job"/>
    <rdfs:range rdf:resource="http://www.w3.org/2001/XMLSchema#string"/>
  </owl:DatatypeProperty>
  <owl:DatatypeProperty rdf:about="http://example.org/onto/prop/google_database_migration_service_migration_job_id">
    <rdfs:label>id</rdfs:label>
    <rdfs:domain rdf:resource="http://example.org/onto/class/google_database_migration_service_migration_job"/>
    <rdfs:range rdf:resource="http://www.w3.org/2001/XMLSchema#string"/>
  </owl:DatatypeProperty>
  <owl:DatatypeProperty rdf:about="http://example.org/onto/prop/google_database_migration_service_migration_job_labels">
    <rdfs:label>labels</rdfs:label>
    <rdfs:comment>The resource labels for migration job to use to annotate any related underlying resources such as Compute Engine VMs.


**Note**: This field is non-authoritative, and will only manage the labels present in your configuration.
Please refer to the field 'effective_labels' for all of the labels present on the resource.</rdfs:comment>
    <rdfs:domain rdf:resource="http://example.org/onto/class/google_database_migration_service_migration_job"/>
    <rdfs:range rdf:resource="http://www.w3.org/2001/XMLSchema#string"/>
  </owl:DatatypeProperty>
  <owl:DatatypeProperty rdf:about="http://example.org/onto/prop/google_database_migration_service_migration_job_location">
    <rdfs:label>location</rdfs:label>
    <rdfs:comment>The location where the migration job should reside.</rdfs:comment>
    <rdfs:domain rdf:resource="http://example.org/onto/class/google_database_migration_service_migration_job"/>
    <rdfs:range rdf:resource="http://www.w3.org/2001/XMLSchema#string"/>
  </owl:DatatypeProperty>
  <owl:DatatypeProperty rdf:about="http://example.org/onto/prop/google_database_migration_service_migration_job_migration_job_id">
    <rdfs:label>migration_job_id</rdfs:label>
    <rdfs:comment>The ID of the migration job.</rdfs:comment>
    <rdfs:domain rdf:resource="http://example.org/onto/class/google_database_migration_service_migration_job"/>
    <rdfs:range rdf:resource="http://www.w3.org/2001/XMLSchema#string"/>
  </owl:DatatypeProperty>
  <owl:DatatypeProperty rdf:about="http://example.org/onto/prop/google_database_migration_service_migration_job_name">
    <rdfs:label>name</rdfs:label>
    <rdfs:comment>The name of this migration job resource in the form of projects/{project}/locations/{location}/migrationJobs/{migrationJob}.</rdfs:comment>
    <rdfs:domain rdf:resource="http://example.org/onto/class/google_database_migration_service_migration_job"/>
    <rdfs:range rdf:resource="http://www.w3.org/2001/XMLSchema#string"/>
  </owl:DatatypeProperty>
  <owl:DatatypeProperty rdf:about="http://example.org/onto/prop/google_database_migration_service_migration_job_phase">
    <rdfs:label>phase</rdfs:label>
    <rdfs:comment>The current migration job phase.</rdfs:comment>
    <rdfs:domain rdf:resource="http://example.org/onto/class/google_database_migration_service_migration_job"/>
    <rdfs:range rdf:resource="http://www.w3.org/2001/XMLSchema#string"/>
  </owl:DatatypeProperty>
  <owl:DatatypeProperty rdf:about="http://example.org/onto/prop/google_database_migration_service_migration_job_project">
    <rdfs:label>project</rdfs:label>
    <rdfs:domain rdf:resource="http://example.org/onto/class/google_database_migration_service_migration_job"/>
    <rdfs:range rdf:resource="http://www.w3.org/2001/XMLSchema#string"/>
  </owl:DatatypeProperty>
  <owl:DatatypeProperty rdf:about="http://example.org/onto/prop/google_database_migration_service_migration_job_source">
    <rdfs:label>source</rdfs:label>
    <rdfs:comment>The name of the source connection profile resource in the form of projects/{project}/locations/{location}/connectionProfiles/{sourceConnectionProfile}.</rdfs:comment>
    <rdfs:domain rdf:resource="http://example.org/onto/class/google_database_migration_service_migration_job"/>
    <rdfs:range rdf:resource="http://www.w3.org/2001/XMLSchema#string"/>
  </owl:DatatypeProperty>
  <owl:DatatypeProperty rdf:about="http://example.org/onto/prop/google_database_migration_service_migration_job_state">
    <rdfs:label>state</rdfs:label>
    <rdfs:comment>The current migration job state.</rdfs:comment>
    <rdfs:domain rdf:resource="http://example.org/onto/class/google_database_migration_service_migration_job"/>
    <rdfs:range rdf:resource="http://www.w3.org/2001/XMLSchema#string"/>
  </owl:DatatypeProperty>
  <owl:DatatypeProperty rdf:about="http://example.org/onto/prop/google_database_migration_service_migration_job_terraform_labels">
    <rdfs:label>terraform_labels</rdfs:label>
    <rdfs:comment>The combination of labels configured directly on the resource
 and default labels configured on the provider.</rdfs:comment>
    <rdfs:domain rdf:resource="http://example.org/onto/class/google_database_migration_service_migration_job"/>
    <rdfs:range rdf:resource="http://www.w3.org/2001/XMLSchema#string"/>
  </owl:DatatypeProperty>
  <owl:DatatypeProperty rdf:about="http://example.org/onto/prop/google_database_migration_service_migration_job_type">
    <rdfs:label>type</rdfs:label>
    <rdfs:comment>The type of the migration job. Possible values: ["ONE_TIME", "CONTINUOUS"]</rdfs:comment>
    <rdfs:domain rdf:resource="http://example.org/onto/class/google_database_migration_service_migration_job"/>
    <rdfs:range rdf:resource="http://www.w3.org/2001/XMLSchema#string"/>
  </owl:DatatypeProperty>
  <owl:DatatypeProperty rdf:about="http://example.org/onto/prop/google_database_migration_service_migration_job_name">
    <rdfs:label>name</rdfs:label>
    <rdfs:comment>The name of the flag</rdfs:comment>
    <rdfs:domain rdf:resource="http://example.org/onto/class/google_database_migration_service_migration_job"/>
    <rdfs:range rdf:resource="http://www.w3.org/2001/XMLSchema#string"/>
  </owl:DatatypeProperty>
  <owl:DatatypeProperty rdf:about="http://example.org/onto/prop/google_database_migration_service_migration_job_value">
    <rdfs:label>value</rdfs:label>
    <rdfs:comment>The vale of the flag</rdfs:comment>
    <rdfs:domain rdf:resource="http://example.org/onto/class/google_database_migration_service_migration_job"/>
    <rdfs:range rdf:resource="http://www.w3.org/2001/XMLSchema#string"/>
  </owl:DatatypeProperty>
  <owl:DatatypeProperty rdf:about="http://example.org/onto/prop/google_database_migration_service_migration_job_dump_parallel_level">
    <rdfs:label>dump_parallel_level</rdfs:label>
    <rdfs:comment>Initial dump parallelism level. Possible values: ["MIN", "OPTIMAL", "MAX"]</rdfs:comment>
    <rdfs:domain rdf:resource="http://example.org/onto/class/google_database_migration_service_migration_job"/>
    <rdfs:range rdf:resource="http://www.w3.org/2001/XMLSchema#string"/>
  </owl:DatatypeProperty>
  <owl:DatatypeProperty rdf:about="http://example.org/onto/prop/google_database_migration_service_migration_job_vm">
    <rdfs:label>vm</rdfs:label>
    <rdfs:comment>The name of the virtual machine (Compute Engine) used as the bastion server
for the SSH tunnel.</rdfs:comment>
    <rdfs:domain rdf:resource="http://example.org/onto/class/google_database_migration_service_migration_job"/>
    <rdfs:range rdf:resource="http://www.w3.org/2001/XMLSchema#string"/>
  </owl:DatatypeProperty>
  <owl:DatatypeProperty rdf:about="http://example.org/onto/prop/google_database_migration_service_migration_job_vm_ip">
    <rdfs:label>vm_ip</rdfs:label>
    <rdfs:comment>The IP of the virtual machine (Compute Engine) used as the bastion server
for the SSH tunnel.</rdfs:comment>
    <rdfs:domain rdf:resource="http://example.org/onto/class/google_database_migration_service_migration_job"/>
    <rdfs:range rdf:resource="http://www.w3.org/2001/XMLSchema#string"/>
  </owl:DatatypeProperty>
  <owl:DatatypeProperty rdf:about="http://example.org/onto/prop/google_database_migration_service_migration_job_vm_port">
    <rdfs:label>vm_port</rdfs:label>
    <rdfs:comment>The forwarding port of the virtual machine (Compute Engine) used as the
bastion server for the SSH tunnel.</rdfs:comment>
    <rdfs:domain rdf:resource="http://example.org/onto/class/google_database_migration_service_migration_job"/>
    <rdfs:range rdf:resource="http://www.w3.org/2001/XMLSchema#string"/>
  </owl:DatatypeProperty>
  <owl:DatatypeProperty rdf:about="http://example.org/onto/prop/google_database_migration_service_migration_job_vpc">
    <rdfs:label>vpc</rdfs:label>
    <rdfs:comment>The name of the VPC to peer with the Cloud SQL private network.</rdfs:comment>
    <rdfs:domain rdf:resource="http://example.org/onto/class/google_database_migration_service_migration_job"/>
    <rdfs:range rdf:resource="http://www.w3.org/2001/XMLSchema#string"/>
  </owl:DatatypeProperty>
  <owl:DatatypeProperty rdf:about="http://example.org/onto/prop/google_database_migration_service_migration_job_create">
    <rdfs:label>create</rdfs:label>
    <rdfs:domain rdf:resource="http://example.org/onto/class/google_database_migration_service_migration_job"/>
    <rdfs:range rdf:resource="http://www.w3.org/2001/XMLSchema#string"/>
  </owl:DatatypeProperty>
  <owl:DatatypeProperty rdf:about="http://example.org/onto/prop/google_database_migration_service_migration_job_delete">
    <rdfs:label>delete</rdfs:label>
    <rdfs:domain rdf:resource="http://example.org/onto/class/google_database_migration_service_migration_job"/>
    <rdfs:range rdf:resource="http://www.w3.org/2001/XMLSchema#string"/>
  </owl:DatatypeProperty>
  <owl:DatatypeProperty rdf:about="http://example.org/onto/prop/google_database_migration_service_migration_job_update">
    <rdfs:label>update</rdfs:label>
    <rdfs:domain rdf:resource="http://example.org/onto/class/google_database_migration_service_migration_job"/>
    <rdfs:range rdf:resource="http://www.w3.org/2001/XMLSchema#string"/>
  </owl:DatatypeProperty>
  <owl:DatatypeProperty rdf:about="http://example.org/onto/prop/google_database_migration_service_migration_job_vpc">
    <rdfs:label>vpc</rdfs:label>
    <rdfs:comment>The name of the VPC network to peer with the Cloud SQL private network.</rdfs:comment>
    <rdfs:domain rdf:resource="http://example.org/onto/class/google_database_migration_service_migration_job"/>
    <rdfs:range rdf:resource="http://www.w3.org/2001/XMLSchema#string"/>
  </owl:DatatypeProperty>
</rdf:RDF>
