<?xml version="1.0" encoding="UTF-8"?>
<rdf:RDF
  xmlns:rdf="http://www.w3.org/1999/02/22-rdf-syntax-ns#"
  xmlns:rdfs="http://www.w3.org/2000/01/rdf-schema#"
  xmlns:owl="http://www.w3.org/2002/07/owl#"
  xmlns:xsd="http://www.w3.org/2001/XMLSchema#"
  xml:base="http://example.org/onto/">
  <owl:Class rdf:about="http://example.org/onto/class/google_data_fusion_instance">
    <rdfs:label>google_data_fusion_instance</rdfs:label>
    <rdfs:comment>#
#     ***     AUTO GENERATED CODE    ***    Type: MMv1     ***
#
# ----------------------------------------------------------------------------
#
#     This code is generated by Magic Modules using the following:
#
#     Configuration: https:#github.com/GoogleCloudPlatform/magic-modules/tree/main/mmv1/products/datafusion/Instance.yaml
#     Template:      https:#github.com/GoogleCloudPlatform/magic-modules/tree/main/mmv1/templates/terraform/resource.html.markdown.tmpl
#
#     DO NOT EDIT this file directly. Any changes made to this file will be
#     overwritten during the next generation cycle.
#
# ----------------------------------------------------------------------------
subcategory: "Cloud Data Fusion"
description: |-
  Represents a Data Fusion instance.
---</rdfs:comment>
  </owl:Class>
  <owl:DatatypeProperty rdf:about="http://example.org/onto/prop/google_data_fusion_instance_api_endpoint">
    <rdfs:label>api_endpoint</rdfs:label>
    <rdfs:comment>Endpoint on which the REST APIs is accessible.</rdfs:comment>
    <rdfs:domain rdf:resource="http://example.org/onto/class/google_data_fusion_instance"/>
    <rdfs:range rdf:resource="http://www.w3.org/2001/XMLSchema#string"/>
  </owl:DatatypeProperty>
  <owl:DatatypeProperty rdf:about="http://example.org/onto/prop/google_data_fusion_instance_create_time">
    <rdfs:label>create_time</rdfs:label>
    <rdfs:comment>The time the instance was created in RFC3339 UTC "Zulu" format, accurate to nanoseconds.</rdfs:comment>
    <rdfs:domain rdf:resource="http://example.org/onto/class/google_data_fusion_instance"/>
    <rdfs:range rdf:resource="http://www.w3.org/2001/XMLSchema#string"/>
  </owl:DatatypeProperty>
  <owl:DatatypeProperty rdf:about="http://example.org/onto/prop/google_data_fusion_instance_dataproc_service_account">
    <rdfs:label>dataproc_service_account</rdfs:label>
    <rdfs:comment>User-managed service account to set on Dataproc when Cloud Data Fusion creates Dataproc to run data processing pipelines.</rdfs:comment>
    <rdfs:domain rdf:resource="http://example.org/onto/class/google_data_fusion_instance"/>
    <rdfs:range rdf:resource="http://www.w3.org/2001/XMLSchema#string"/>
  </owl:DatatypeProperty>
  <owl:DatatypeProperty rdf:about="http://example.org/onto/prop/google_data_fusion_instance_description">
    <rdfs:label>description</rdfs:label>
    <rdfs:comment>An optional description of the instance.</rdfs:comment>
    <rdfs:domain rdf:resource="http://example.org/onto/class/google_data_fusion_instance"/>
    <rdfs:range rdf:resource="http://www.w3.org/2001/XMLSchema#string"/>
  </owl:DatatypeProperty>
  <owl:DatatypeProperty rdf:about="http://example.org/onto/prop/google_data_fusion_instance_display_name">
    <rdfs:label>display_name</rdfs:label>
    <rdfs:comment>Display name for an instance.</rdfs:comment>
    <rdfs:domain rdf:resource="http://example.org/onto/class/google_data_fusion_instance"/>
    <rdfs:range rdf:resource="http://www.w3.org/2001/XMLSchema#string"/>
  </owl:DatatypeProperty>
  <owl:DatatypeProperty rdf:about="http://example.org/onto/prop/google_data_fusion_instance_effective_labels">
    <rdfs:label>effective_labels</rdfs:label>
    <rdfs:comment>All of labels (key/value pairs) present on the resource in GCP, including the labels configured through Terraform, other clients and services.</rdfs:comment>
    <rdfs:domain rdf:resource="http://example.org/onto/class/google_data_fusion_instance"/>
    <rdfs:range rdf:resource="http://www.w3.org/2001/XMLSchema#string"/>
  </owl:DatatypeProperty>
  <owl:DatatypeProperty rdf:about="http://example.org/onto/prop/google_data_fusion_instance_enable_rbac">
    <rdfs:label>enable_rbac</rdfs:label>
    <rdfs:comment>Option to enable granular role-based access control.</rdfs:comment>
    <rdfs:domain rdf:resource="http://example.org/onto/class/google_data_fusion_instance"/>
    <rdfs:range rdf:resource="http://www.w3.org/2001/XMLSchema#string"/>
  </owl:DatatypeProperty>
  <owl:DatatypeProperty rdf:about="http://example.org/onto/prop/google_data_fusion_instance_enable_stackdriver_logging">
    <rdfs:label>enable_stackdriver_logging</rdfs:label>
    <rdfs:comment>Option to enable Stackdriver Logging.</rdfs:comment>
    <rdfs:domain rdf:resource="http://example.org/onto/class/google_data_fusion_instance"/>
    <rdfs:range rdf:resource="http://www.w3.org/2001/XMLSchema#string"/>
  </owl:DatatypeProperty>
  <owl:DatatypeProperty rdf:about="http://example.org/onto/prop/google_data_fusion_instance_enable_stackdriver_monitoring">
    <rdfs:label>enable_stackdriver_monitoring</rdfs:label>
    <rdfs:comment>Option to enable Stackdriver Monitoring.</rdfs:comment>
    <rdfs:domain rdf:resource="http://example.org/onto/class/google_data_fusion_instance"/>
    <rdfs:range rdf:resource="http://www.w3.org/2001/XMLSchema#string"/>
  </owl:DatatypeProperty>
  <owl:DatatypeProperty rdf:about="http://example.org/onto/prop/google_data_fusion_instance_gcs_bucket">
    <rdfs:label>gcs_bucket</rdfs:label>
    <rdfs:comment>Cloud Storage bucket generated by Data Fusion in the customer project.</rdfs:comment>
    <rdfs:domain rdf:resource="http://example.org/onto/class/google_data_fusion_instance"/>
    <rdfs:range rdf:resource="http://www.w3.org/2001/XMLSchema#string"/>
  </owl:DatatypeProperty>
  <owl:DatatypeProperty rdf:about="http://example.org/onto/prop/google_data_fusion_instance_id">
    <rdfs:label>id</rdfs:label>
    <rdfs:domain rdf:resource="http://example.org/onto/class/google_data_fusion_instance"/>
    <rdfs:range rdf:resource="http://www.w3.org/2001/XMLSchema#string"/>
  </owl:DatatypeProperty>
  <owl:DatatypeProperty rdf:about="http://example.org/onto/prop/google_data_fusion_instance_labels">
    <rdfs:label>labels</rdfs:label>
    <rdfs:comment>The resource labels for instance to use to annotate any related underlying resources,
such as Compute Engine VMs.


**Note**: This field is non-authoritative, and will only manage the labels present in your configuration.
Please refer to the field 'effective_labels' for all of the labels present on the resource.</rdfs:comment>
    <rdfs:domain rdf:resource="http://example.org/onto/class/google_data_fusion_instance"/>
    <rdfs:range rdf:resource="http://www.w3.org/2001/XMLSchema#string"/>
  </owl:DatatypeProperty>
  <owl:DatatypeProperty rdf:about="http://example.org/onto/prop/google_data_fusion_instance_name">
    <rdfs:label>name</rdfs:label>
    <rdfs:comment>The ID of the instance or a fully qualified identifier for the instance.</rdfs:comment>
    <rdfs:domain rdf:resource="http://example.org/onto/class/google_data_fusion_instance"/>
    <rdfs:range rdf:resource="http://www.w3.org/2001/XMLSchema#string"/>
  </owl:DatatypeProperty>
  <owl:DatatypeProperty rdf:about="http://example.org/onto/prop/google_data_fusion_instance_options">
    <rdfs:label>options</rdfs:label>
    <rdfs:comment>Map of additional options used to configure the behavior of Data Fusion instance.</rdfs:comment>
    <rdfs:domain rdf:resource="http://example.org/onto/class/google_data_fusion_instance"/>
    <rdfs:range rdf:resource="http://www.w3.org/2001/XMLSchema#string"/>
  </owl:DatatypeProperty>
  <owl:DatatypeProperty rdf:about="http://example.org/onto/prop/google_data_fusion_instance_p4_service_account">
    <rdfs:label>p4_service_account</rdfs:label>
    <rdfs:comment>P4 service account for the customer project.</rdfs:comment>
    <rdfs:domain rdf:resource="http://example.org/onto/class/google_data_fusion_instance"/>
    <rdfs:range rdf:resource="http://www.w3.org/2001/XMLSchema#string"/>
  </owl:DatatypeProperty>
  <owl:DatatypeProperty rdf:about="http://example.org/onto/prop/google_data_fusion_instance_private_instance">
    <rdfs:label>private_instance</rdfs:label>
    <rdfs:comment>Specifies whether the Data Fusion instance should be private. If set to
true, all Data Fusion nodes will have private IP addresses and will not be
able to access the public internet.</rdfs:comment>
    <rdfs:domain rdf:resource="http://example.org/onto/class/google_data_fusion_instance"/>
    <rdfs:range rdf:resource="http://www.w3.org/2001/XMLSchema#string"/>
  </owl:DatatypeProperty>
  <owl:DatatypeProperty rdf:about="http://example.org/onto/prop/google_data_fusion_instance_project">
    <rdfs:label>project</rdfs:label>
    <rdfs:domain rdf:resource="http://example.org/onto/class/google_data_fusion_instance"/>
    <rdfs:range rdf:resource="http://www.w3.org/2001/XMLSchema#string"/>
  </owl:DatatypeProperty>
  <owl:DatatypeProperty rdf:about="http://example.org/onto/prop/google_data_fusion_instance_region">
    <rdfs:label>region</rdfs:label>
    <rdfs:comment>The region of the Data Fusion instance.</rdfs:comment>
    <rdfs:domain rdf:resource="http://example.org/onto/class/google_data_fusion_instance"/>
    <rdfs:range rdf:resource="http://www.w3.org/2001/XMLSchema#string"/>
  </owl:DatatypeProperty>
  <owl:DatatypeProperty rdf:about="http://example.org/onto/prop/google_data_fusion_instance_service_endpoint">
    <rdfs:label>service_endpoint</rdfs:label>
    <rdfs:comment>Endpoint on which the Data Fusion UI and REST APIs are accessible.</rdfs:comment>
    <rdfs:domain rdf:resource="http://example.org/onto/class/google_data_fusion_instance"/>
    <rdfs:range rdf:resource="http://www.w3.org/2001/XMLSchema#string"/>
  </owl:DatatypeProperty>
  <owl:DatatypeProperty rdf:about="http://example.org/onto/prop/google_data_fusion_instance_state">
    <rdfs:label>state</rdfs:label>
    <rdfs:comment>The current state of this Data Fusion instance.
- CREATING: Instance is being created
- RUNNING: Instance is running and ready for requests
- FAILED: Instance creation failed
- DELETING: Instance is being deleted
- UPGRADING: Instance is being upgraded
- RESTARTING: Instance is being restarted</rdfs:comment>
    <rdfs:domain rdf:resource="http://example.org/onto/class/google_data_fusion_instance"/>
    <rdfs:range rdf:resource="http://www.w3.org/2001/XMLSchema#string"/>
  </owl:DatatypeProperty>
  <owl:DatatypeProperty rdf:about="http://example.org/onto/prop/google_data_fusion_instance_state_message">
    <rdfs:label>state_message</rdfs:label>
    <rdfs:comment>Additional information about the current state of this Data Fusion instance if available.</rdfs:comment>
    <rdfs:domain rdf:resource="http://example.org/onto/class/google_data_fusion_instance"/>
    <rdfs:range rdf:resource="http://www.w3.org/2001/XMLSchema#string"/>
  </owl:DatatypeProperty>
  <owl:DatatypeProperty rdf:about="http://example.org/onto/prop/google_data_fusion_instance_tags">
    <rdfs:label>tags</rdfs:label>
    <rdfs:comment>A map of resource manager tags.
Resource manager tag keys and values have the same definition as resource manager tags.
Keys must be in the format tagKeys/{tag_key_id}, and values are in the format tagValues/{tag_value_id}.
The field is ignored (both PUT & PATCH) when empty.</rdfs:comment>
    <rdfs:domain rdf:resource="http://example.org/onto/class/google_data_fusion_instance"/>
    <rdfs:range rdf:resource="http://www.w3.org/2001/XMLSchema#string"/>
  </owl:DatatypeProperty>
  <owl:DatatypeProperty rdf:about="http://example.org/onto/prop/google_data_fusion_instance_tenant_project_id">
    <rdfs:label>tenant_project_id</rdfs:label>
    <rdfs:comment>The name of the tenant project.</rdfs:comment>
    <rdfs:domain rdf:resource="http://example.org/onto/class/google_data_fusion_instance"/>
    <rdfs:range rdf:resource="http://www.w3.org/2001/XMLSchema#string"/>
  </owl:DatatypeProperty>
  <owl:DatatypeProperty rdf:about="http://example.org/onto/prop/google_data_fusion_instance_terraform_labels">
    <rdfs:label>terraform_labels</rdfs:label>
    <rdfs:comment>The combination of labels configured directly on the resource
 and default labels configured on the provider.</rdfs:comment>
    <rdfs:domain rdf:resource="http://example.org/onto/class/google_data_fusion_instance"/>
    <rdfs:range rdf:resource="http://www.w3.org/2001/XMLSchema#string"/>
  </owl:DatatypeProperty>
  <owl:DatatypeProperty rdf:about="http://example.org/onto/prop/google_data_fusion_instance_type">
    <rdfs:label>type</rdfs:label>
    <rdfs:comment>Represents the type of Data Fusion instance. Each type is configured with
the default settings for processing and memory.
- BASIC: Basic Data Fusion instance. In Basic type, the user will be able to create data pipelines
using point and click UI. However, there are certain limitations, such as fewer number
of concurrent pipelines, no support for streaming pipelines, etc.
- ENTERPRISE: Enterprise Data Fusion instance. In Enterprise type, the user will have more features
available, such as support for streaming pipelines, higher number of concurrent pipelines, etc.
- DEVELOPER: Developer Data Fusion instance. In Developer type, the user will have all features available but
with restrictive capabilities. This is to help enterprises design and develop their data ingestion and integration
pipelines at low cost. Possible values: ["BASIC", "ENTERPRISE", "DEVELOPER"]</rdfs:comment>
    <rdfs:domain rdf:resource="http://example.org/onto/class/google_data_fusion_instance"/>
    <rdfs:range rdf:resource="http://www.w3.org/2001/XMLSchema#string"/>
  </owl:DatatypeProperty>
  <owl:DatatypeProperty rdf:about="http://example.org/onto/prop/google_data_fusion_instance_update_time">
    <rdfs:label>update_time</rdfs:label>
    <rdfs:comment>The time the instance was last updated in RFC3339 UTC "Zulu" format, accurate to nanoseconds.</rdfs:comment>
    <rdfs:domain rdf:resource="http://example.org/onto/class/google_data_fusion_instance"/>
    <rdfs:range rdf:resource="http://www.w3.org/2001/XMLSchema#string"/>
  </owl:DatatypeProperty>
  <owl:DatatypeProperty rdf:about="http://example.org/onto/prop/google_data_fusion_instance_version">
    <rdfs:label>version</rdfs:label>
    <rdfs:comment>Current version of the Data Fusion.</rdfs:comment>
    <rdfs:domain rdf:resource="http://example.org/onto/class/google_data_fusion_instance"/>
    <rdfs:range rdf:resource="http://www.w3.org/2001/XMLSchema#string"/>
  </owl:DatatypeProperty>
  <owl:DatatypeProperty rdf:about="http://example.org/onto/prop/google_data_fusion_instance_zone">
    <rdfs:label>zone</rdfs:label>
    <rdfs:comment>Name of the zone in which the Data Fusion instance will be created. Only DEVELOPER instances use this field.</rdfs:comment>
    <rdfs:domain rdf:resource="http://example.org/onto/class/google_data_fusion_instance"/>
    <rdfs:range rdf:resource="http://www.w3.org/2001/XMLSchema#string"/>
  </owl:DatatypeProperty>
  <owl:DatatypeProperty rdf:about="http://example.org/onto/prop/google_data_fusion_instance_accelerator_type">
    <rdfs:label>accelerator_type</rdfs:label>
    <rdfs:comment>The type of an accelator for a CDF instance. Possible values: ["CDC", "HEALTHCARE", "CCAI_INSIGHTS"]</rdfs:comment>
    <rdfs:domain rdf:resource="http://example.org/onto/class/google_data_fusion_instance"/>
    <rdfs:range rdf:resource="http://www.w3.org/2001/XMLSchema#string"/>
  </owl:DatatypeProperty>
  <owl:DatatypeProperty rdf:about="http://example.org/onto/prop/google_data_fusion_instance_state">
    <rdfs:label>state</rdfs:label>
    <rdfs:comment>The type of an accelator for a CDF instance. Possible values: ["ENABLED", "DISABLED"]</rdfs:comment>
    <rdfs:domain rdf:resource="http://example.org/onto/class/google_data_fusion_instance"/>
    <rdfs:range rdf:resource="http://www.w3.org/2001/XMLSchema#string"/>
  </owl:DatatypeProperty>
  <owl:DatatypeProperty rdf:about="http://example.org/onto/prop/google_data_fusion_instance_key_reference">
    <rdfs:label>key_reference</rdfs:label>
    <rdfs:comment>The name of the key which is used to encrypt/decrypt customer data. For key in Cloud KMS, the key should be in the format of projects/*/locations/*/keyRings/*/cryptoKeys/*.</rdfs:comment>
    <rdfs:domain rdf:resource="http://example.org/onto/class/google_data_fusion_instance"/>
    <rdfs:range rdf:resource="http://www.w3.org/2001/XMLSchema#string"/>
  </owl:DatatypeProperty>
  <owl:DatatypeProperty rdf:about="http://example.org/onto/prop/google_data_fusion_instance_enabled">
    <rdfs:label>enabled</rdfs:label>
    <rdfs:comment>Option to enable Event Publishing.</rdfs:comment>
    <rdfs:domain rdf:resource="http://example.org/onto/class/google_data_fusion_instance"/>
    <rdfs:range rdf:resource="http://www.w3.org/2001/XMLSchema#string"/>
  </owl:DatatypeProperty>
  <owl:DatatypeProperty rdf:about="http://example.org/onto/prop/google_data_fusion_instance_topic">
    <rdfs:label>topic</rdfs:label>
    <rdfs:comment>The resource name of the Pub/Sub topic. Format: projects/{projectId}/topics/{topic_id}</rdfs:comment>
    <rdfs:domain rdf:resource="http://example.org/onto/class/google_data_fusion_instance"/>
    <rdfs:range rdf:resource="http://www.w3.org/2001/XMLSchema#string"/>
  </owl:DatatypeProperty>
  <owl:DatatypeProperty rdf:about="http://example.org/onto/prop/google_data_fusion_instance_connection_type">
    <rdfs:label>connection_type</rdfs:label>
    <rdfs:comment>Optional. Type of connection for establishing private IP connectivity between the Data Fusion customer project VPC and
the corresponding tenant project from a predefined list of available connection modes.
If this field is unspecified for a private instance, VPC peering is used. Possible values: ["VPC_PEERING", "PRIVATE_SERVICE_CONNECT_INTERFACES"]</rdfs:comment>
    <rdfs:domain rdf:resource="http://example.org/onto/class/google_data_fusion_instance"/>
    <rdfs:range rdf:resource="http://www.w3.org/2001/XMLSchema#string"/>
  </owl:DatatypeProperty>
  <owl:DatatypeProperty rdf:about="http://example.org/onto/prop/google_data_fusion_instance_ip_allocation">
    <rdfs:label>ip_allocation</rdfs:label>
    <rdfs:comment>The IP range in CIDR notation to use for the managed Data Fusion instance
nodes. This range must not overlap with any other ranges used in the Data Fusion instance network.</rdfs:comment>
    <rdfs:domain rdf:resource="http://example.org/onto/class/google_data_fusion_instance"/>
    <rdfs:range rdf:resource="http://www.w3.org/2001/XMLSchema#string"/>
  </owl:DatatypeProperty>
  <owl:DatatypeProperty rdf:about="http://example.org/onto/prop/google_data_fusion_instance_network">
    <rdfs:label>network</rdfs:label>
    <rdfs:comment>Name of the network in the project with which the tenant project
will be peered for executing pipelines. In case of shared VPC where the network resides in another host
project the network should specified in the form of projects/{host-project-id}/global/networks/{network}</rdfs:comment>
    <rdfs:domain rdf:resource="http://example.org/onto/class/google_data_fusion_instance"/>
    <rdfs:range rdf:resource="http://www.w3.org/2001/XMLSchema#string"/>
  </owl:DatatypeProperty>
  <owl:DatatypeProperty rdf:about="http://example.org/onto/prop/google_data_fusion_instance_effective_unreachable_cidr_block">
    <rdfs:label>effective_unreachable_cidr_block</rdfs:label>
    <rdfs:comment>Output only. The CIDR block to which the CDF instance can't route traffic to in the consumer project VPC.
The size of this block is /25. The format of this field is governed by RFC 4632.</rdfs:comment>
    <rdfs:domain rdf:resource="http://example.org/onto/class/google_data_fusion_instance"/>
    <rdfs:range rdf:resource="http://www.w3.org/2001/XMLSchema#string"/>
  </owl:DatatypeProperty>
  <owl:DatatypeProperty rdf:about="http://example.org/onto/prop/google_data_fusion_instance_network_attachment">
    <rdfs:label>network_attachment</rdfs:label>
    <rdfs:comment>Optional. The reference to the network attachment used to establish private connectivity.
It will be of the form projects/{project-id}/regions/{region}/networkAttachments/{network-attachment-id}.
This is required only when using connection type PRIVATE_SERVICE_CONNECT_INTERFACES.</rdfs:comment>
    <rdfs:domain rdf:resource="http://example.org/onto/class/google_data_fusion_instance"/>
    <rdfs:range rdf:resource="http://www.w3.org/2001/XMLSchema#string"/>
  </owl:DatatypeProperty>
  <owl:DatatypeProperty rdf:about="http://example.org/onto/prop/google_data_fusion_instance_unreachable_cidr_block">
    <rdfs:label>unreachable_cidr_block</rdfs:label>
    <rdfs:comment>Optional. Input only. The CIDR block to which the CDF instance can't route traffic to in the consumer project VPC.
The size of this block should be at least /25. This range should not overlap with the primary address range of any subnetwork used by the network attachment.
This range can be used for other purposes in the consumer VPC as long as there is no requirement for CDF to reach destinations using these addresses.
If this value is not provided, the server chooses a non RFC 1918 address range. The format of this field is governed by RFC 4632.</rdfs:comment>
    <rdfs:domain rdf:resource="http://example.org/onto/class/google_data_fusion_instance"/>
    <rdfs:range rdf:resource="http://www.w3.org/2001/XMLSchema#string"/>
  </owl:DatatypeProperty>
  <owl:DatatypeProperty rdf:about="http://example.org/onto/prop/google_data_fusion_instance_create">
    <rdfs:label>create</rdfs:label>
    <rdfs:domain rdf:resource="http://example.org/onto/class/google_data_fusion_instance"/>
    <rdfs:range rdf:resource="http://www.w3.org/2001/XMLSchema#string"/>
  </owl:DatatypeProperty>
  <owl:DatatypeProperty rdf:about="http://example.org/onto/prop/google_data_fusion_instance_delete">
    <rdfs:label>delete</rdfs:label>
    <rdfs:domain rdf:resource="http://example.org/onto/class/google_data_fusion_instance"/>
    <rdfs:range rdf:resource="http://www.w3.org/2001/XMLSchema#string"/>
  </owl:DatatypeProperty>
  <owl:DatatypeProperty rdf:about="http://example.org/onto/prop/google_data_fusion_instance_update">
    <rdfs:label>update</rdfs:label>
    <rdfs:domain rdf:resource="http://example.org/onto/class/google_data_fusion_instance"/>
    <rdfs:range rdf:resource="http://www.w3.org/2001/XMLSchema#string"/>
  </owl:DatatypeProperty>
</rdf:RDF>
