<?xml version="1.0" encoding="UTF-8"?>
<rdf:RDF
  xmlns:rdf="http://www.w3.org/1999/02/22-rdf-syntax-ns#"
  xmlns:rdfs="http://www.w3.org/2000/01/rdf-schema#"
  xmlns:owl="http://www.w3.org/2002/07/owl#"
  xmlns:xsd="http://www.w3.org/2001/XMLSchema#"
  xml:base="http://example.org/onto/">
  <owl:Class rdf:about="http://example.org/onto/class/google_compute_forwarding_rule">
    <rdfs:label>google_compute_forwarding_rule</rdfs:label>
    <rdfs:comment>#
#     ***     AUTO GENERATED CODE    ***    Type: MMv1     ***
#
# ----------------------------------------------------------------------------
#
#     This code is generated by Magic Modules using the following:
#
#     Configuration: https:#github.com/GoogleCloudPlatform/magic-modules/tree/main/mmv1/products/compute/ForwardingRule.yaml
#     Template:      https:#github.com/GoogleCloudPlatform/magic-modules/tree/main/mmv1/templates/terraform/resource.html.markdown.tmpl
#
#     DO NOT EDIT this file directly. Any changes made to this file will be
#     overwritten during the next generation cycle.
#
# ----------------------------------------------------------------------------
subcategory: "Compute Engine"
description: |-
  A ForwardingRule resource.
---</rdfs:comment>
  </owl:Class>
  <owl:DatatypeProperty rdf:about="http://example.org/onto/prop/google_compute_forwarding_rule_all_ports">
    <rdfs:label>all_ports</rdfs:label>
    <rdfs:comment>The 'ports', 'portRange', and 'allPorts' fields are mutually exclusive.
Only packets addressed to ports in the specified range will be forwarded
to the backends configured with this forwarding rule.

The 'allPorts' field has the following limitations:
* It requires that the forwarding rule 'IPProtocol' be TCP, UDP, SCTP, or
L3_DEFAULT.
* It's applicable only to the following products: internal passthrough
Network Load Balancers, backend service-based external passthrough Network
Load Balancers, and internal and external protocol forwarding.
* Set this field to true to allow packets addressed to any port or packets
lacking destination port information (for example, UDP fragments after the
first fragment) to be forwarded to the backends configured with this
forwarding rule. The L3_DEFAULT protocol requires 'allPorts' be set to
true.</rdfs:comment>
    <rdfs:domain rdf:resource="http://example.org/onto/class/google_compute_forwarding_rule"/>
    <rdfs:range rdf:resource="http://www.w3.org/2001/XMLSchema#string"/>
  </owl:DatatypeProperty>
  <owl:DatatypeProperty rdf:about="http://example.org/onto/prop/google_compute_forwarding_rule_allow_global_access">
    <rdfs:label>allow_global_access</rdfs:label>
    <rdfs:comment>This field is used along with the 'backend_service' field for
internal load balancing or with the 'target' field for internal
TargetInstance.

If the field is set to 'TRUE', clients can access ILB from all
regions.

Otherwise only allows access from clients in the same region as the
internal load balancer.</rdfs:comment>
    <rdfs:domain rdf:resource="http://example.org/onto/class/google_compute_forwarding_rule"/>
    <rdfs:range rdf:resource="http://www.w3.org/2001/XMLSchema#string"/>
  </owl:DatatypeProperty>
  <owl:DatatypeProperty rdf:about="http://example.org/onto/prop/google_compute_forwarding_rule_allow_psc_global_access">
    <rdfs:label>allow_psc_global_access</rdfs:label>
    <rdfs:comment>This is used in PSC consumer ForwardingRule to control whether the PSC endpoint can be accessed from another region.</rdfs:comment>
    <rdfs:domain rdf:resource="http://example.org/onto/class/google_compute_forwarding_rule"/>
    <rdfs:range rdf:resource="http://www.w3.org/2001/XMLSchema#string"/>
  </owl:DatatypeProperty>
  <owl:DatatypeProperty rdf:about="http://example.org/onto/prop/google_compute_forwarding_rule_backend_service">
    <rdfs:label>backend_service</rdfs:label>
    <rdfs:comment>Identifies the backend service to which the forwarding rule sends traffic.

Required for Internal TCP/UDP Load Balancing and Network Load Balancing;
must be omitted for all other load balancer types.</rdfs:comment>
    <rdfs:domain rdf:resource="http://example.org/onto/class/google_compute_forwarding_rule"/>
    <rdfs:range rdf:resource="http://www.w3.org/2001/XMLSchema#string"/>
  </owl:DatatypeProperty>
  <owl:DatatypeProperty rdf:about="http://example.org/onto/prop/google_compute_forwarding_rule_base_forwarding_rule">
    <rdfs:label>base_forwarding_rule</rdfs:label>
    <rdfs:comment>[Output Only] The URL for the corresponding base Forwarding Rule. By base Forwarding Rule, we mean the Forwarding Rule that has the same IP address, protocol, and port settings with the current Forwarding Rule, but without sourceIPRanges specified. Always empty if the current Forwarding Rule does not have sourceIPRanges specified.</rdfs:comment>
    <rdfs:domain rdf:resource="http://example.org/onto/class/google_compute_forwarding_rule"/>
    <rdfs:range rdf:resource="http://www.w3.org/2001/XMLSchema#string"/>
  </owl:DatatypeProperty>
  <owl:DatatypeProperty rdf:about="http://example.org/onto/prop/google_compute_forwarding_rule_creation_timestamp">
    <rdfs:label>creation_timestamp</rdfs:label>
    <rdfs:comment>Creation timestamp in RFC3339 text format.</rdfs:comment>
    <rdfs:domain rdf:resource="http://example.org/onto/class/google_compute_forwarding_rule"/>
    <rdfs:range rdf:resource="http://www.w3.org/2001/XMLSchema#string"/>
  </owl:DatatypeProperty>
  <owl:DatatypeProperty rdf:about="http://example.org/onto/prop/google_compute_forwarding_rule_description">
    <rdfs:label>description</rdfs:label>
    <rdfs:comment>An optional description of this resource. Provide this property when
you create the resource.</rdfs:comment>
    <rdfs:domain rdf:resource="http://example.org/onto/class/google_compute_forwarding_rule"/>
    <rdfs:range rdf:resource="http://www.w3.org/2001/XMLSchema#string"/>
  </owl:DatatypeProperty>
  <owl:DatatypeProperty rdf:about="http://example.org/onto/prop/google_compute_forwarding_rule_effective_labels">
    <rdfs:label>effective_labels</rdfs:label>
    <rdfs:comment>All of labels (key/value pairs) present on the resource in GCP, including the labels configured through Terraform, other clients and services.</rdfs:comment>
    <rdfs:domain rdf:resource="http://example.org/onto/class/google_compute_forwarding_rule"/>
    <rdfs:range rdf:resource="http://www.w3.org/2001/XMLSchema#string"/>
  </owl:DatatypeProperty>
  <owl:DatatypeProperty rdf:about="http://example.org/onto/prop/google_compute_forwarding_rule_forwarding_rule_id">
    <rdfs:label>forwarding_rule_id</rdfs:label>
    <rdfs:comment>The unique identifier number for the resource. This identifier is defined by the server.</rdfs:comment>
    <rdfs:domain rdf:resource="http://example.org/onto/class/google_compute_forwarding_rule"/>
    <rdfs:range rdf:resource="http://www.w3.org/2001/XMLSchema#string"/>
  </owl:DatatypeProperty>
  <owl:DatatypeProperty rdf:about="http://example.org/onto/prop/google_compute_forwarding_rule_id">
    <rdfs:label>id</rdfs:label>
    <rdfs:domain rdf:resource="http://example.org/onto/class/google_compute_forwarding_rule"/>
    <rdfs:range rdf:resource="http://www.w3.org/2001/XMLSchema#string"/>
  </owl:DatatypeProperty>
  <owl:DatatypeProperty rdf:about="http://example.org/onto/prop/google_compute_forwarding_rule_ip_address">
    <rdfs:label>ip_address</rdfs:label>
    <rdfs:comment>IP address for which this forwarding rule accepts traffic. When a client
sends traffic to this IP address, the forwarding rule directs the traffic
to the referenced 'target' or 'backendService'.

While creating a forwarding rule, specifying an 'IPAddress' is
required under the following circumstances:

* When the 'target' is set to 'targetGrpcProxy' and
'validateForProxyless' is set to 'true', the
'IPAddress' should be set to '0.0.0.0'.
* When the 'target' is a Private Service Connect Google APIs
bundle, you must specify an 'IPAddress'.

Otherwise, you can optionally specify an IP address that references an
existing static (reserved) IP address resource. When omitted, Google Cloud
assigns an ephemeral IP address.

Use one of the following formats to specify an IP address while creating a
forwarding rule:

* IP address number, as in '100.1.2.3'
* IPv6 address range, as in '2600:1234::/96'
* Full resource URL, as in
'https://www.googleapis.com/compute/v1/projects/project_id/regions/region/addresses/address-name'
* Partial URL or by name, as in:
  * 'projects/project_id/regions/region/addresses/address-name'
  * 'regions/region/addresses/address-name'
  * 'global/addresses/address-name'
  * 'address-name'

The forwarding rule's 'target' or 'backendService',
and in most cases, also the 'loadBalancingScheme', determine the
type of IP address that you can use. For detailed information, see
[IP address
specifications](https://cloud.google.com/load-balancing/docs/forwarding-rule-concepts#ip_address_specifications).

When reading an 'IPAddress', the API always returns the IP
address number.</rdfs:comment>
    <rdfs:domain rdf:resource="http://example.org/onto/class/google_compute_forwarding_rule"/>
    <rdfs:range rdf:resource="http://www.w3.org/2001/XMLSchema#string"/>
  </owl:DatatypeProperty>
  <owl:DatatypeProperty rdf:about="http://example.org/onto/prop/google_compute_forwarding_rule_ip_collection">
    <rdfs:label>ip_collection</rdfs:label>
    <rdfs:comment>Resource reference of a PublicDelegatedPrefix. The PDP must be a sub-PDP
in EXTERNAL_IPV6_FORWARDING_RULE_CREATION mode.
Use one of the following formats to specify a sub-PDP when creating an
IPv6 NetLB forwarding rule using BYOIP:
Full resource URL, as in:
  * 'https://www.googleapis.com/compute/v1/projects/{{projectId}}/regions/{{region}}/publicDelegatedPrefixes/{{sub-pdp-name}}'
Partial URL, as in:
  * 'projects/{{projectId}}/regions/region/publicDelegatedPrefixes/{{sub-pdp-name}}'
  * 'regions/{{region}}/publicDelegatedPrefixes/{{sub-pdp-name}}'</rdfs:comment>
    <rdfs:domain rdf:resource="http://example.org/onto/class/google_compute_forwarding_rule"/>
    <rdfs:range rdf:resource="http://www.w3.org/2001/XMLSchema#string"/>
  </owl:DatatypeProperty>
  <owl:DatatypeProperty rdf:about="http://example.org/onto/prop/google_compute_forwarding_rule_ip_protocol">
    <rdfs:label>ip_protocol</rdfs:label>
    <rdfs:comment>The IP protocol to which this rule applies.

For protocol forwarding, valid
options are 'TCP', 'UDP', 'ESP',
'AH', 'SCTP', 'ICMP' and
'L3_DEFAULT'.

The valid IP protocols are different for different load balancing products
as described in [Load balancing
features](https://cloud.google.com/load-balancing/docs/features#protocols_from_the_load_balancer_to_the_backends).

A Forwarding Rule with protocol L3_DEFAULT can attach with target instance or
backend service with UNSPECIFIED protocol.
A forwarding rule with "L3_DEFAULT" IPProtocal cannot be attached to a backend service with TCP or UDP. Possible values: ["TCP", "UDP", "ESP", "AH", "SCTP", "ICMP", "L3_DEFAULT"]</rdfs:comment>
    <rdfs:domain rdf:resource="http://example.org/onto/class/google_compute_forwarding_rule"/>
    <rdfs:range rdf:resource="http://www.w3.org/2001/XMLSchema#string"/>
  </owl:DatatypeProperty>
  <owl:DatatypeProperty rdf:about="http://example.org/onto/prop/google_compute_forwarding_rule_ip_version">
    <rdfs:label>ip_version</rdfs:label>
    <rdfs:comment>The IP address version that will be used by this forwarding rule.
Valid options are IPV4 and IPV6.

If not set, the IPv4 address will be used by default. Possible values: ["IPV4", "IPV6"]</rdfs:comment>
    <rdfs:domain rdf:resource="http://example.org/onto/class/google_compute_forwarding_rule"/>
    <rdfs:range rdf:resource="http://www.w3.org/2001/XMLSchema#string"/>
  </owl:DatatypeProperty>
  <owl:DatatypeProperty rdf:about="http://example.org/onto/prop/google_compute_forwarding_rule_is_mirroring_collector">
    <rdfs:label>is_mirroring_collector</rdfs:label>
    <rdfs:comment>Indicates whether or not this load balancer can be used as a collector for
packet mirroring. To prevent mirroring loops, instances behind this
load balancer will not have their traffic mirrored even if a
'PacketMirroring' rule applies to them.

This can only be set to true for load balancers that have their
'loadBalancingScheme' set to 'INTERNAL'.</rdfs:comment>
    <rdfs:domain rdf:resource="http://example.org/onto/class/google_compute_forwarding_rule"/>
    <rdfs:range rdf:resource="http://www.w3.org/2001/XMLSchema#string"/>
  </owl:DatatypeProperty>
  <owl:DatatypeProperty rdf:about="http://example.org/onto/prop/google_compute_forwarding_rule_label_fingerprint">
    <rdfs:label>label_fingerprint</rdfs:label>
    <rdfs:comment>The fingerprint used for optimistic locking of this resource.  Used
internally during updates.</rdfs:comment>
    <rdfs:domain rdf:resource="http://example.org/onto/class/google_compute_forwarding_rule"/>
    <rdfs:range rdf:resource="http://www.w3.org/2001/XMLSchema#string"/>
  </owl:DatatypeProperty>
  <owl:DatatypeProperty rdf:about="http://example.org/onto/prop/google_compute_forwarding_rule_labels">
    <rdfs:label>labels</rdfs:label>
    <rdfs:comment>Labels to apply to this forwarding rule.  A list of key->value pairs.


**Note**: This field is non-authoritative, and will only manage the labels present in your configuration.
Please refer to the field 'effective_labels' for all of the labels present on the resource.</rdfs:comment>
    <rdfs:domain rdf:resource="http://example.org/onto/class/google_compute_forwarding_rule"/>
    <rdfs:range rdf:resource="http://www.w3.org/2001/XMLSchema#string"/>
  </owl:DatatypeProperty>
  <owl:DatatypeProperty rdf:about="http://example.org/onto/prop/google_compute_forwarding_rule_load_balancing_scheme">
    <rdfs:label>load_balancing_scheme</rdfs:label>
    <rdfs:comment>Specifies the forwarding rule type.

Note that an empty string value ('""') is also supported for some use
cases, for example PSC (private service connection) regional forwarding
rules.

For more information about forwarding rules, refer to
[Forwarding rule concepts](https://cloud.google.com/load-balancing/docs/forwarding-rule-concepts). Default value: "EXTERNAL" Possible values: ["EXTERNAL", "EXTERNAL_MANAGED", "INTERNAL", "INTERNAL_MANAGED"]</rdfs:comment>
    <rdfs:domain rdf:resource="http://example.org/onto/class/google_compute_forwarding_rule"/>
    <rdfs:range rdf:resource="http://www.w3.org/2001/XMLSchema#string"/>
  </owl:DatatypeProperty>
  <owl:DatatypeProperty rdf:about="http://example.org/onto/prop/google_compute_forwarding_rule_name">
    <rdfs:label>name</rdfs:label>
    <rdfs:comment>Name of the resource; provided by the client when the resource is created.
The name must be 1-63 characters long, and comply with
[RFC1035](https://www.ietf.org/rfc/rfc1035.txt).

Specifically, the name must be 1-63 characters long and match the regular
expression '[a-z]([-a-z0-9]*[a-z0-9])?' which means the first
character must be a lowercase letter, and all following characters must
be a dash, lowercase letter, or digit, except the last character, which
cannot be a dash.

For Private Service Connect forwarding rules that forward traffic to Google
APIs, the forwarding rule name must be a 1-20 characters string with
lowercase letters and numbers and must start with a letter.</rdfs:comment>
    <rdfs:domain rdf:resource="http://example.org/onto/class/google_compute_forwarding_rule"/>
    <rdfs:range rdf:resource="http://www.w3.org/2001/XMLSchema#string"/>
  </owl:DatatypeProperty>
  <owl:DatatypeProperty rdf:about="http://example.org/onto/prop/google_compute_forwarding_rule_network">
    <rdfs:label>network</rdfs:label>
    <rdfs:comment>This field is not used for external load balancing.

For Internal TCP/UDP Load Balancing, this field identifies the network that
the load balanced IP should belong to for this Forwarding Rule.
If the subnetwork is specified, the network of the subnetwork will be used.
If neither subnetwork nor this field is specified, the default network will
be used.

For Private Service Connect forwarding rules that forward traffic to Google
APIs, a network must be provided.</rdfs:comment>
    <rdfs:domain rdf:resource="http://example.org/onto/class/google_compute_forwarding_rule"/>
    <rdfs:range rdf:resource="http://www.w3.org/2001/XMLSchema#string"/>
  </owl:DatatypeProperty>
  <owl:DatatypeProperty rdf:about="http://example.org/onto/prop/google_compute_forwarding_rule_network_tier">
    <rdfs:label>network_tier</rdfs:label>
    <rdfs:comment>This signifies the networking tier used for configuring
this load balancer and can only take the following values:
'PREMIUM', 'STANDARD'.

For regional ForwardingRule, the valid values are 'PREMIUM' and
'STANDARD'. For GlobalForwardingRule, the valid value is
'PREMIUM'.

If this field is not specified, it is assumed to be 'PREMIUM'.
If 'IPAddress' is specified, this value must be equal to the
networkTier of the Address. Possible values: ["PREMIUM", "STANDARD"]</rdfs:comment>
    <rdfs:domain rdf:resource="http://example.org/onto/class/google_compute_forwarding_rule"/>
    <rdfs:range rdf:resource="http://www.w3.org/2001/XMLSchema#string"/>
  </owl:DatatypeProperty>
  <owl:DatatypeProperty rdf:about="http://example.org/onto/prop/google_compute_forwarding_rule_no_automate_dns_zone">
    <rdfs:label>no_automate_dns_zone</rdfs:label>
    <rdfs:comment>This is used in PSC consumer ForwardingRule to control whether it should try to auto-generate a DNS zone or not. Non-PSC forwarding rules do not use this field.</rdfs:comment>
    <rdfs:domain rdf:resource="http://example.org/onto/class/google_compute_forwarding_rule"/>
    <rdfs:range rdf:resource="http://www.w3.org/2001/XMLSchema#string"/>
  </owl:DatatypeProperty>
  <owl:DatatypeProperty rdf:about="http://example.org/onto/prop/google_compute_forwarding_rule_port_range">
    <rdfs:label>port_range</rdfs:label>
    <rdfs:comment>The 'ports', 'portRange', and 'allPorts' fields are mutually exclusive.
Only packets addressed to ports in the specified range will be forwarded
to the backends configured with this forwarding rule.

The 'portRange' field has the following limitations:
* It requires that the forwarding rule 'IPProtocol' be TCP, UDP, or SCTP,
and
* It's applicable only to the following products: external passthrough
Network Load Balancers, internal and external proxy Network Load
Balancers, internal and external Application Load Balancers, external
protocol forwarding, and Classic VPN.
* Some products have restrictions on what ports can be used. See
[port specifications](https://cloud.google.com/load-balancing/docs/forwarding-rule-concepts#port_specifications)
for details.

For external forwarding rules, two or more forwarding rules cannot use the
same '[IPAddress, IPProtocol]' pair, and cannot have overlapping
'portRange's.

For internal forwarding rules within the same VPC network, two or more
forwarding rules cannot use the same '[IPAddress, IPProtocol]' pair, and
cannot have overlapping 'portRange's.

@pattern: \d+(?:-\d+)?</rdfs:comment>
    <rdfs:domain rdf:resource="http://example.org/onto/class/google_compute_forwarding_rule"/>
    <rdfs:range rdf:resource="http://www.w3.org/2001/XMLSchema#string"/>
  </owl:DatatypeProperty>
  <owl:DatatypeProperty rdf:about="http://example.org/onto/prop/google_compute_forwarding_rule_ports">
    <rdfs:label>ports</rdfs:label>
    <rdfs:comment>The 'ports', 'portRange', and 'allPorts' fields are mutually exclusive.
Only packets addressed to ports in the specified range will be forwarded
to the backends configured with this forwarding rule.

The 'ports' field has the following limitations:
* It requires that the forwarding rule 'IPProtocol' be TCP, UDP, or SCTP,
and
* It's applicable only to the following products: internal passthrough
Network Load Balancers, backend service-based external passthrough Network
Load Balancers, and internal protocol forwarding.
* You can specify a list of up to five ports by number, separated by
commas. The ports can be contiguous or discontiguous.

For external forwarding rules, two or more forwarding rules cannot use the
same '[IPAddress, IPProtocol]' pair if they share at least one port
number.

For internal forwarding rules within the same VPC network, two or more
forwarding rules cannot use the same '[IPAddress, IPProtocol]' pair if
they share at least one port number.

@pattern: \d+(?:-\d+)?</rdfs:comment>
    <rdfs:domain rdf:resource="http://example.org/onto/class/google_compute_forwarding_rule"/>
    <rdfs:range rdf:resource="http://www.w3.org/2001/XMLSchema#string"/>
  </owl:DatatypeProperty>
  <owl:DatatypeProperty rdf:about="http://example.org/onto/prop/google_compute_forwarding_rule_project">
    <rdfs:label>project</rdfs:label>
    <rdfs:domain rdf:resource="http://example.org/onto/class/google_compute_forwarding_rule"/>
    <rdfs:range rdf:resource="http://www.w3.org/2001/XMLSchema#string"/>
  </owl:DatatypeProperty>
  <owl:DatatypeProperty rdf:about="http://example.org/onto/prop/google_compute_forwarding_rule_psc_connection_id">
    <rdfs:label>psc_connection_id</rdfs:label>
    <rdfs:comment>The PSC connection id of the PSC Forwarding Rule.</rdfs:comment>
    <rdfs:domain rdf:resource="http://example.org/onto/class/google_compute_forwarding_rule"/>
    <rdfs:range rdf:resource="http://www.w3.org/2001/XMLSchema#string"/>
  </owl:DatatypeProperty>
  <owl:DatatypeProperty rdf:about="http://example.org/onto/prop/google_compute_forwarding_rule_psc_connection_status">
    <rdfs:label>psc_connection_status</rdfs:label>
    <rdfs:comment>The PSC connection status of the PSC Forwarding Rule. Possible values: 'STATUS_UNSPECIFIED', 'PENDING', 'ACCEPTED', 'REJECTED', 'CLOSED'</rdfs:comment>
    <rdfs:domain rdf:resource="http://example.org/onto/class/google_compute_forwarding_rule"/>
    <rdfs:range rdf:resource="http://www.w3.org/2001/XMLSchema#string"/>
  </owl:DatatypeProperty>
  <owl:DatatypeProperty rdf:about="http://example.org/onto/prop/google_compute_forwarding_rule_recreate_closed_psc">
    <rdfs:label>recreate_closed_psc</rdfs:label>
    <rdfs:comment>This is used in PSC consumer ForwardingRule to make terraform recreate the ForwardingRule when the status is closed</rdfs:comment>
    <rdfs:domain rdf:resource="http://example.org/onto/class/google_compute_forwarding_rule"/>
    <rdfs:range rdf:resource="http://www.w3.org/2001/XMLSchema#string"/>
  </owl:DatatypeProperty>
  <owl:DatatypeProperty rdf:about="http://example.org/onto/prop/google_compute_forwarding_rule_region">
    <rdfs:label>region</rdfs:label>
    <rdfs:comment>A reference to the region where the regional forwarding rule resides.

This field is not applicable to global forwarding rules.</rdfs:comment>
    <rdfs:domain rdf:resource="http://example.org/onto/class/google_compute_forwarding_rule"/>
    <rdfs:range rdf:resource="http://www.w3.org/2001/XMLSchema#string"/>
  </owl:DatatypeProperty>
  <owl:DatatypeProperty rdf:about="http://example.org/onto/prop/google_compute_forwarding_rule_self_link">
    <rdfs:label>self_link</rdfs:label>
    <rdfs:domain rdf:resource="http://example.org/onto/class/google_compute_forwarding_rule"/>
    <rdfs:range rdf:resource="http://www.w3.org/2001/XMLSchema#string"/>
  </owl:DatatypeProperty>
  <owl:DatatypeProperty rdf:about="http://example.org/onto/prop/google_compute_forwarding_rule_service_label">
    <rdfs:label>service_label</rdfs:label>
    <rdfs:comment>An optional prefix to the service name for this Forwarding Rule.
If specified, will be the first label of the fully qualified service
name.

The label must be 1-63 characters long, and comply with RFC1035.
Specifically, the label must be 1-63 characters long and match the
regular expression '[a-z]([-a-z0-9]*[a-z0-9])?' which means the first
character must be a lowercase letter, and all following characters
must be a dash, lowercase letter, or digit, except the last
character, which cannot be a dash.

This field is only used for INTERNAL load balancing.</rdfs:comment>
    <rdfs:domain rdf:resource="http://example.org/onto/class/google_compute_forwarding_rule"/>
    <rdfs:range rdf:resource="http://www.w3.org/2001/XMLSchema#string"/>
  </owl:DatatypeProperty>
  <owl:DatatypeProperty rdf:about="http://example.org/onto/prop/google_compute_forwarding_rule_service_name">
    <rdfs:label>service_name</rdfs:label>
    <rdfs:comment>The internal fully qualified service name for this Forwarding Rule.

This field is only used for INTERNAL load balancing.</rdfs:comment>
    <rdfs:domain rdf:resource="http://example.org/onto/class/google_compute_forwarding_rule"/>
    <rdfs:range rdf:resource="http://www.w3.org/2001/XMLSchema#string"/>
  </owl:DatatypeProperty>
  <owl:DatatypeProperty rdf:about="http://example.org/onto/prop/google_compute_forwarding_rule_source_ip_ranges">
    <rdfs:label>source_ip_ranges</rdfs:label>
    <rdfs:comment>If not empty, this Forwarding Rule will only forward the traffic when the source IP address matches one of the IP addresses or CIDR ranges set here. Note that a Forwarding Rule can only have up to 64 source IP ranges, and this field can only be used with a regional Forwarding Rule whose scheme is EXTERNAL. Each sourceIpRange entry should be either an IP address (for example, 1.2.3.4) or a CIDR range (for example, 1.2.3.0/24).</rdfs:comment>
    <rdfs:domain rdf:resource="http://example.org/onto/class/google_compute_forwarding_rule"/>
    <rdfs:range rdf:resource="http://www.w3.org/2001/XMLSchema#string"/>
  </owl:DatatypeProperty>
  <owl:DatatypeProperty rdf:about="http://example.org/onto/prop/google_compute_forwarding_rule_subnetwork">
    <rdfs:label>subnetwork</rdfs:label>
    <rdfs:comment>This field identifies the subnetwork that the load balanced IP should
belong to for this Forwarding Rule, used in internal load balancing and
network load balancing with IPv6.

If the network specified is in auto subnet mode, this field is optional.
However, a subnetwork must be specified if the network is in custom subnet
mode or when creating external forwarding rule with IPv6.</rdfs:comment>
    <rdfs:domain rdf:resource="http://example.org/onto/class/google_compute_forwarding_rule"/>
    <rdfs:range rdf:resource="http://www.w3.org/2001/XMLSchema#string"/>
  </owl:DatatypeProperty>
  <owl:DatatypeProperty rdf:about="http://example.org/onto/prop/google_compute_forwarding_rule_target">
    <rdfs:label>target</rdfs:label>
    <rdfs:comment>The URL of the target resource to receive the matched traffic.  For
regional forwarding rules, this target must be in the same region as the
forwarding rule. For global forwarding rules, this target must be a global
load balancing resource.

The forwarded traffic must be of a type appropriate to the target object.
*  For load balancers, see the "Target" column in [Port specifications](https://cloud.google.com/load-balancing/docs/forwarding-rule-concepts#ip_address_specifications).

For Private Service Connect forwarding rules that forward traffic to managed services, the target must be a service attachment.</rdfs:comment>
    <rdfs:domain rdf:resource="http://example.org/onto/class/google_compute_forwarding_rule"/>
    <rdfs:range rdf:resource="http://www.w3.org/2001/XMLSchema#string"/>
  </owl:DatatypeProperty>
  <owl:DatatypeProperty rdf:about="http://example.org/onto/prop/google_compute_forwarding_rule_terraform_labels">
    <rdfs:label>terraform_labels</rdfs:label>
    <rdfs:comment>The combination of labels configured directly on the resource
 and default labels configured on the provider.</rdfs:comment>
    <rdfs:domain rdf:resource="http://example.org/onto/class/google_compute_forwarding_rule"/>
    <rdfs:range rdf:resource="http://www.w3.org/2001/XMLSchema#string"/>
  </owl:DatatypeProperty>
  <owl:DatatypeProperty rdf:about="http://example.org/onto/prop/google_compute_forwarding_rule_namespace">
    <rdfs:label>namespace</rdfs:label>
    <rdfs:comment>Service Directory namespace to register the forwarding rule under.</rdfs:comment>
    <rdfs:domain rdf:resource="http://example.org/onto/class/google_compute_forwarding_rule"/>
    <rdfs:range rdf:resource="http://www.w3.org/2001/XMLSchema#string"/>
  </owl:DatatypeProperty>
  <owl:DatatypeProperty rdf:about="http://example.org/onto/prop/google_compute_forwarding_rule_service">
    <rdfs:label>service</rdfs:label>
    <rdfs:comment>Service Directory service to register the forwarding rule under.</rdfs:comment>
    <rdfs:domain rdf:resource="http://example.org/onto/class/google_compute_forwarding_rule"/>
    <rdfs:range rdf:resource="http://www.w3.org/2001/XMLSchema#string"/>
  </owl:DatatypeProperty>
  <owl:DatatypeProperty rdf:about="http://example.org/onto/prop/google_compute_forwarding_rule_create">
    <rdfs:label>create</rdfs:label>
    <rdfs:domain rdf:resource="http://example.org/onto/class/google_compute_forwarding_rule"/>
    <rdfs:range rdf:resource="http://www.w3.org/2001/XMLSchema#string"/>
  </owl:DatatypeProperty>
  <owl:DatatypeProperty rdf:about="http://example.org/onto/prop/google_compute_forwarding_rule_delete">
    <rdfs:label>delete</rdfs:label>
    <rdfs:domain rdf:resource="http://example.org/onto/class/google_compute_forwarding_rule"/>
    <rdfs:range rdf:resource="http://www.w3.org/2001/XMLSchema#string"/>
  </owl:DatatypeProperty>
  <owl:DatatypeProperty rdf:about="http://example.org/onto/prop/google_compute_forwarding_rule_update">
    <rdfs:label>update</rdfs:label>
    <rdfs:domain rdf:resource="http://example.org/onto/class/google_compute_forwarding_rule"/>
    <rdfs:range rdf:resource="http://www.w3.org/2001/XMLSchema#string"/>
  </owl:DatatypeProperty>
</rdf:RDF>
