<?xml version="1.0" encoding="UTF-8"?>
<rdf:RDF
  xmlns:rdf="http://www.w3.org/1999/02/22-rdf-syntax-ns#"
  xmlns:rdfs="http://www.w3.org/2000/01/rdf-schema#"
  xmlns:owl="http://www.w3.org/2002/07/owl#"
  xmlns:xsd="http://www.w3.org/2001/XMLSchema#"
  xml:base="http://example.org/onto/">
  <owl:Class rdf:about="http://example.org/onto/class/google_biglake_database">
    <rdfs:label>google_biglake_database</rdfs:label>
    <rdfs:comment>#
#     ***     AUTO GENERATED CODE    ***    Type: MMv1     ***
#
# ----------------------------------------------------------------------------
#
#     This code is generated by Magic Modules using the following:
#
#     Configuration: https:#github.com/GoogleCloudPlatform/magic-modules/tree/main/mmv1/products/biglake/Database.yaml
#     Template:      https:#github.com/GoogleCloudPlatform/magic-modules/tree/main/mmv1/templates/terraform/resource.html.markdown.tmpl
#
#     DO NOT EDIT this file directly. Any changes made to this file will be
#     overwritten during the next generation cycle.
#
# ----------------------------------------------------------------------------
subcategory: "Biglake"
description: |-
  Databases are containers of tables.
---</rdfs:comment>
  </owl:Class>
  <owl:DatatypeProperty rdf:about="http://example.org/onto/prop/google_biglake_database_catalog">
    <rdfs:label>catalog</rdfs:label>
    <rdfs:comment>The parent catalog.</rdfs:comment>
    <rdfs:domain rdf:resource="http://example.org/onto/class/google_biglake_database"/>
    <rdfs:range rdf:resource="http://www.w3.org/2001/XMLSchema#string"/>
  </owl:DatatypeProperty>
  <owl:DatatypeProperty rdf:about="http://example.org/onto/prop/google_biglake_database_create_time">
    <rdfs:label>create_time</rdfs:label>
    <rdfs:comment>Output only. The creation time of the database. A timestamp in RFC3339
UTC "Zulu" format, with nanosecond resolution and up to nine fractional
digits. Examples: "2014-10-02T15:01:23Z" and
"2014-10-02T15:01:23.045123456Z".</rdfs:comment>
    <rdfs:domain rdf:resource="http://example.org/onto/class/google_biglake_database"/>
    <rdfs:range rdf:resource="http://www.w3.org/2001/XMLSchema#string"/>
  </owl:DatatypeProperty>
  <owl:DatatypeProperty rdf:about="http://example.org/onto/prop/google_biglake_database_delete_time">
    <rdfs:label>delete_time</rdfs:label>
    <rdfs:comment>Output only. The deletion time of the database. Only set after the
database is deleted. A timestamp in RFC3339 UTC "Zulu" format, with
nanosecond resolution and up to nine fractional digits. Examples:
"2014-10-02T15:01:23Z" and "2014-10-02T15:01:23.045123456Z".</rdfs:comment>
    <rdfs:domain rdf:resource="http://example.org/onto/class/google_biglake_database"/>
    <rdfs:range rdf:resource="http://www.w3.org/2001/XMLSchema#string"/>
  </owl:DatatypeProperty>
  <owl:DatatypeProperty rdf:about="http://example.org/onto/prop/google_biglake_database_expire_time">
    <rdfs:label>expire_time</rdfs:label>
    <rdfs:comment>Output only. The time when this database is considered expired. Only set
after the database is deleted. A timestamp in RFC3339 UTC "Zulu" format,
with nanosecond resolution and up to nine fractional digits. Examples:
"2014-10-02T15:01:23Z" and "2014-10-02T15:01:23.045123456Z".</rdfs:comment>
    <rdfs:domain rdf:resource="http://example.org/onto/class/google_biglake_database"/>
    <rdfs:range rdf:resource="http://www.w3.org/2001/XMLSchema#string"/>
  </owl:DatatypeProperty>
  <owl:DatatypeProperty rdf:about="http://example.org/onto/prop/google_biglake_database_id">
    <rdfs:label>id</rdfs:label>
    <rdfs:domain rdf:resource="http://example.org/onto/class/google_biglake_database"/>
    <rdfs:range rdf:resource="http://www.w3.org/2001/XMLSchema#string"/>
  </owl:DatatypeProperty>
  <owl:DatatypeProperty rdf:about="http://example.org/onto/prop/google_biglake_database_name">
    <rdfs:label>name</rdfs:label>
    <rdfs:comment>The name of the database.</rdfs:comment>
    <rdfs:domain rdf:resource="http://example.org/onto/class/google_biglake_database"/>
    <rdfs:range rdf:resource="http://www.w3.org/2001/XMLSchema#string"/>
  </owl:DatatypeProperty>
  <owl:DatatypeProperty rdf:about="http://example.org/onto/prop/google_biglake_database_type">
    <rdfs:label>type</rdfs:label>
    <rdfs:comment>The database type.</rdfs:comment>
    <rdfs:domain rdf:resource="http://example.org/onto/class/google_biglake_database"/>
    <rdfs:range rdf:resource="http://www.w3.org/2001/XMLSchema#string"/>
  </owl:DatatypeProperty>
  <owl:DatatypeProperty rdf:about="http://example.org/onto/prop/google_biglake_database_update_time">
    <rdfs:label>update_time</rdfs:label>
    <rdfs:comment>Output only. The last modification time of the database. A timestamp in
RFC3339 UTC "Zulu" format, with nanosecond resolution and up to nine
fractional digits. Examples: "2014-10-02T15:01:23Z" and
"2014-10-02T15:01:23.045123456Z".</rdfs:comment>
    <rdfs:domain rdf:resource="http://example.org/onto/class/google_biglake_database"/>
    <rdfs:range rdf:resource="http://www.w3.org/2001/XMLSchema#string"/>
  </owl:DatatypeProperty>
  <owl:DatatypeProperty rdf:about="http://example.org/onto/prop/google_biglake_database_location_uri">
    <rdfs:label>location_uri</rdfs:label>
    <rdfs:comment>Cloud Storage folder URI where the database data is stored, starting with "gs://".</rdfs:comment>
    <rdfs:domain rdf:resource="http://example.org/onto/class/google_biglake_database"/>
    <rdfs:range rdf:resource="http://www.w3.org/2001/XMLSchema#string"/>
  </owl:DatatypeProperty>
  <owl:DatatypeProperty rdf:about="http://example.org/onto/prop/google_biglake_database_parameters">
    <rdfs:label>parameters</rdfs:label>
    <rdfs:comment>Stores user supplied Hive database parameters. An object containing a
list of"key": value pairs.
Example: { "name": "wrench", "mass": "1.3kg", "count": "3" }.</rdfs:comment>
    <rdfs:domain rdf:resource="http://example.org/onto/class/google_biglake_database"/>
    <rdfs:range rdf:resource="http://www.w3.org/2001/XMLSchema#string"/>
  </owl:DatatypeProperty>
  <owl:DatatypeProperty rdf:about="http://example.org/onto/prop/google_biglake_database_create">
    <rdfs:label>create</rdfs:label>
    <rdfs:domain rdf:resource="http://example.org/onto/class/google_biglake_database"/>
    <rdfs:range rdf:resource="http://www.w3.org/2001/XMLSchema#string"/>
  </owl:DatatypeProperty>
  <owl:DatatypeProperty rdf:about="http://example.org/onto/prop/google_biglake_database_delete">
    <rdfs:label>delete</rdfs:label>
    <rdfs:domain rdf:resource="http://example.org/onto/class/google_biglake_database"/>
    <rdfs:range rdf:resource="http://www.w3.org/2001/XMLSchema#string"/>
  </owl:DatatypeProperty>
  <owl:DatatypeProperty rdf:about="http://example.org/onto/prop/google_biglake_database_update">
    <rdfs:label>update</rdfs:label>
    <rdfs:domain rdf:resource="http://example.org/onto/class/google_biglake_database"/>
    <rdfs:range rdf:resource="http://www.w3.org/2001/XMLSchema#string"/>
  </owl:DatatypeProperty>
</rdf:RDF>
