<?xml version="1.0" encoding="UTF-8"?>
<rdf:RDF
  xmlns:rdf="http://www.w3.org/1999/02/22-rdf-syntax-ns#"
  xmlns:rdfs="http://www.w3.org/2000/01/rdf-schema#"
  xmlns:owl="http://www.w3.org/2002/07/owl#"
  xmlns:xsd="http://www.w3.org/2001/XMLSchema#"
  xml:base="http://example.org/onto/">
  <owl:Class rdf:about="http://example.org/onto/class/google_scc_folder_custom_module">
    <rdfs:label>google_scc_folder_custom_module</rdfs:label>
    <rdfs:comment>#
#     ***     AUTO GENERATED CODE    ***    Type: MMv1     ***
#
# ----------------------------------------------------------------------------
#
#     This code is generated by Magic Modules using the following:
#
#     Configuration: https:#github.com/GoogleCloudPlatform/magic-modules/tree/main/mmv1/products/securitycenter/FolderCustomModule.yaml
#     Template:      https:#github.com/GoogleCloudPlatform/magic-modules/tree/main/mmv1/templates/terraform/resource.html.markdown.tmpl
#
#     DO NOT EDIT this file directly. Any changes made to this file will be
#     overwritten during the next generation cycle.
#
# ----------------------------------------------------------------------------
subcategory: "Security Command Center (SCC)"
description: |-
  Represents an instance of a Security Health Analytics custom module, including
  its full module name, display name, enablement state, and last updated time.
---</rdfs:comment>
  </owl:Class>
  <owl:DatatypeProperty rdf:about="http://example.org/onto/prop/google_scc_folder_custom_module_ancestor_module">
    <rdfs:label>ancestor_module</rdfs:label>
    <rdfs:comment>If empty, indicates that the custom module was created in the organization, folder,
or project in which you are viewing the custom module. Otherwise, ancestor_module
specifies the organization or folder from which the custom module is inherited.</rdfs:comment>
    <rdfs:domain rdf:resource="http://example.org/onto/class/google_scc_folder_custom_module"/>
    <rdfs:range rdf:resource="http://www.w3.org/2001/XMLSchema#string"/>
  </owl:DatatypeProperty>
  <owl:DatatypeProperty rdf:about="http://example.org/onto/prop/google_scc_folder_custom_module_display_name">
    <rdfs:label>display_name</rdfs:label>
    <rdfs:comment>The display name of the Security Health Analytics custom module. This
display name becomes the finding category for all findings that are
returned by this custom module. The display name must be between 1 and
128 characters, start with a lowercase letter, and contain alphanumeric
characters or underscores only.</rdfs:comment>
    <rdfs:domain rdf:resource="http://example.org/onto/class/google_scc_folder_custom_module"/>
    <rdfs:range rdf:resource="http://www.w3.org/2001/XMLSchema#string"/>
  </owl:DatatypeProperty>
  <owl:DatatypeProperty rdf:about="http://example.org/onto/prop/google_scc_folder_custom_module_enablement_state">
    <rdfs:label>enablement_state</rdfs:label>
    <rdfs:comment>The enablement state of the custom module. Possible values: ["ENABLED", "DISABLED"]</rdfs:comment>
    <rdfs:domain rdf:resource="http://example.org/onto/class/google_scc_folder_custom_module"/>
    <rdfs:range rdf:resource="http://www.w3.org/2001/XMLSchema#string"/>
  </owl:DatatypeProperty>
  <owl:DatatypeProperty rdf:about="http://example.org/onto/prop/google_scc_folder_custom_module_folder">
    <rdfs:label>folder</rdfs:label>
    <rdfs:comment>Numerical ID of the parent folder.</rdfs:comment>
    <rdfs:domain rdf:resource="http://example.org/onto/class/google_scc_folder_custom_module"/>
    <rdfs:range rdf:resource="http://www.w3.org/2001/XMLSchema#string"/>
  </owl:DatatypeProperty>
  <owl:DatatypeProperty rdf:about="http://example.org/onto/prop/google_scc_folder_custom_module_id">
    <rdfs:label>id</rdfs:label>
    <rdfs:domain rdf:resource="http://example.org/onto/class/google_scc_folder_custom_module"/>
    <rdfs:range rdf:resource="http://www.w3.org/2001/XMLSchema#string"/>
  </owl:DatatypeProperty>
  <owl:DatatypeProperty rdf:about="http://example.org/onto/prop/google_scc_folder_custom_module_last_editor">
    <rdfs:label>last_editor</rdfs:label>
    <rdfs:comment>The editor that last updated the custom module.</rdfs:comment>
    <rdfs:domain rdf:resource="http://example.org/onto/class/google_scc_folder_custom_module"/>
    <rdfs:range rdf:resource="http://www.w3.org/2001/XMLSchema#string"/>
  </owl:DatatypeProperty>
  <owl:DatatypeProperty rdf:about="http://example.org/onto/prop/google_scc_folder_custom_module_name">
    <rdfs:label>name</rdfs:label>
    <rdfs:comment>The resource name of the custom module. Its format is "folders/{folder_id}/securityHealthAnalyticsSettings/customModules/{customModule}".
The id {customModule} is server-generated and is not user settable. It will be a numeric id containing 1-20 digits.</rdfs:comment>
    <rdfs:domain rdf:resource="http://example.org/onto/class/google_scc_folder_custom_module"/>
    <rdfs:range rdf:resource="http://www.w3.org/2001/XMLSchema#string"/>
  </owl:DatatypeProperty>
  <owl:DatatypeProperty rdf:about="http://example.org/onto/prop/google_scc_folder_custom_module_update_time">
    <rdfs:label>update_time</rdfs:label>
    <rdfs:comment>The time at which the custom module was last updated.

A timestamp in RFC3339 UTC "Zulu" format, with nanosecond resolution and
up to nine fractional digits. Examples: "2014-10-02T15:01:23Z" and "2014-10-02T15:01:23.045123456Z".</rdfs:comment>
    <rdfs:domain rdf:resource="http://example.org/onto/class/google_scc_folder_custom_module"/>
    <rdfs:range rdf:resource="http://www.w3.org/2001/XMLSchema#string"/>
  </owl:DatatypeProperty>
  <owl:DatatypeProperty rdf:about="http://example.org/onto/prop/google_scc_folder_custom_module_description">
    <rdfs:label>description</rdfs:label>
    <rdfs:comment>Text that describes the vulnerability or misconfiguration that the custom
module detects. This explanation is returned with each finding instance to
help investigators understand the detected issue. The text must be enclosed in quotation marks.</rdfs:comment>
    <rdfs:domain rdf:resource="http://example.org/onto/class/google_scc_folder_custom_module"/>
    <rdfs:range rdf:resource="http://www.w3.org/2001/XMLSchema#string"/>
  </owl:DatatypeProperty>
  <owl:DatatypeProperty rdf:about="http://example.org/onto/prop/google_scc_folder_custom_module_recommendation">
    <rdfs:label>recommendation</rdfs:label>
    <rdfs:comment>An explanation of the recommended steps that security teams can take to resolve
the detected issue. This explanation is returned with each finding generated by
this module in the nextSteps property of the finding JSON.</rdfs:comment>
    <rdfs:domain rdf:resource="http://example.org/onto/class/google_scc_folder_custom_module"/>
    <rdfs:range rdf:resource="http://www.w3.org/2001/XMLSchema#string"/>
  </owl:DatatypeProperty>
  <owl:DatatypeProperty rdf:about="http://example.org/onto/prop/google_scc_folder_custom_module_severity">
    <rdfs:label>severity</rdfs:label>
    <rdfs:comment>The severity to assign to findings generated by the module. Possible values: ["CRITICAL", "HIGH", "MEDIUM", "LOW"]</rdfs:comment>
    <rdfs:domain rdf:resource="http://example.org/onto/class/google_scc_folder_custom_module"/>
    <rdfs:range rdf:resource="http://www.w3.org/2001/XMLSchema#string"/>
  </owl:DatatypeProperty>
  <owl:DatatypeProperty rdf:about="http://example.org/onto/prop/google_scc_folder_custom_module_name">
    <rdfs:label>name</rdfs:label>
    <rdfs:comment>Name of the property for the custom output.</rdfs:comment>
    <rdfs:domain rdf:resource="http://example.org/onto/class/google_scc_folder_custom_module"/>
    <rdfs:range rdf:resource="http://www.w3.org/2001/XMLSchema#string"/>
  </owl:DatatypeProperty>
  <owl:DatatypeProperty rdf:about="http://example.org/onto/prop/google_scc_folder_custom_module_description">
    <rdfs:label>description</rdfs:label>
    <rdfs:comment>Description of the expression. This is a longer text which describes the
expression, e.g. when hovered over it in a UI.</rdfs:comment>
    <rdfs:domain rdf:resource="http://example.org/onto/class/google_scc_folder_custom_module"/>
    <rdfs:range rdf:resource="http://www.w3.org/2001/XMLSchema#string"/>
  </owl:DatatypeProperty>
  <owl:DatatypeProperty rdf:about="http://example.org/onto/prop/google_scc_folder_custom_module_expression">
    <rdfs:label>expression</rdfs:label>
    <rdfs:comment>Textual representation of an expression in Common Expression Language syntax.</rdfs:comment>
    <rdfs:domain rdf:resource="http://example.org/onto/class/google_scc_folder_custom_module"/>
    <rdfs:range rdf:resource="http://www.w3.org/2001/XMLSchema#string"/>
  </owl:DatatypeProperty>
  <owl:DatatypeProperty rdf:about="http://example.org/onto/prop/google_scc_folder_custom_module_location">
    <rdfs:label>location</rdfs:label>
    <rdfs:comment>String indicating the location of the expression for error reporting, e.g. a
file name and a position in the file.</rdfs:comment>
    <rdfs:domain rdf:resource="http://example.org/onto/class/google_scc_folder_custom_module"/>
    <rdfs:range rdf:resource="http://www.w3.org/2001/XMLSchema#string"/>
  </owl:DatatypeProperty>
  <owl:DatatypeProperty rdf:about="http://example.org/onto/prop/google_scc_folder_custom_module_title">
    <rdfs:label>title</rdfs:label>
    <rdfs:comment>Title for the expression, i.e. a short string describing its purpose. This can
be used e.g. in UIs which allow to enter the expression.</rdfs:comment>
    <rdfs:domain rdf:resource="http://example.org/onto/class/google_scc_folder_custom_module"/>
    <rdfs:range rdf:resource="http://www.w3.org/2001/XMLSchema#string"/>
  </owl:DatatypeProperty>
  <owl:DatatypeProperty rdf:about="http://example.org/onto/prop/google_scc_folder_custom_module_description">
    <rdfs:label>description</rdfs:label>
    <rdfs:comment>Description of the expression. This is a longer text which describes the
expression, e.g. when hovered over it in a UI.</rdfs:comment>
    <rdfs:domain rdf:resource="http://example.org/onto/class/google_scc_folder_custom_module"/>
    <rdfs:range rdf:resource="http://www.w3.org/2001/XMLSchema#string"/>
  </owl:DatatypeProperty>
  <owl:DatatypeProperty rdf:about="http://example.org/onto/prop/google_scc_folder_custom_module_expression">
    <rdfs:label>expression</rdfs:label>
    <rdfs:comment>Textual representation of an expression in Common Expression Language syntax.</rdfs:comment>
    <rdfs:domain rdf:resource="http://example.org/onto/class/google_scc_folder_custom_module"/>
    <rdfs:range rdf:resource="http://www.w3.org/2001/XMLSchema#string"/>
  </owl:DatatypeProperty>
  <owl:DatatypeProperty rdf:about="http://example.org/onto/prop/google_scc_folder_custom_module_location">
    <rdfs:label>location</rdfs:label>
    <rdfs:comment>String indicating the location of the expression for error reporting, e.g. a
file name and a position in the file.</rdfs:comment>
    <rdfs:domain rdf:resource="http://example.org/onto/class/google_scc_folder_custom_module"/>
    <rdfs:range rdf:resource="http://www.w3.org/2001/XMLSchema#string"/>
  </owl:DatatypeProperty>
  <owl:DatatypeProperty rdf:about="http://example.org/onto/prop/google_scc_folder_custom_module_title">
    <rdfs:label>title</rdfs:label>
    <rdfs:comment>Title for the expression, i.e. a short string describing its purpose. This can
be used e.g. in UIs which allow to enter the expression.</rdfs:comment>
    <rdfs:domain rdf:resource="http://example.org/onto/class/google_scc_folder_custom_module"/>
    <rdfs:range rdf:resource="http://www.w3.org/2001/XMLSchema#string"/>
  </owl:DatatypeProperty>
  <owl:DatatypeProperty rdf:about="http://example.org/onto/prop/google_scc_folder_custom_module_resource_types">
    <rdfs:label>resource_types</rdfs:label>
    <rdfs:comment>The resource types to run the detector on.</rdfs:comment>
    <rdfs:domain rdf:resource="http://example.org/onto/class/google_scc_folder_custom_module"/>
    <rdfs:range rdf:resource="http://www.w3.org/2001/XMLSchema#string"/>
  </owl:DatatypeProperty>
  <owl:DatatypeProperty rdf:about="http://example.org/onto/prop/google_scc_folder_custom_module_create">
    <rdfs:label>create</rdfs:label>
    <rdfs:domain rdf:resource="http://example.org/onto/class/google_scc_folder_custom_module"/>
    <rdfs:range rdf:resource="http://www.w3.org/2001/XMLSchema#string"/>
  </owl:DatatypeProperty>
  <owl:DatatypeProperty rdf:about="http://example.org/onto/prop/google_scc_folder_custom_module_delete">
    <rdfs:label>delete</rdfs:label>
    <rdfs:domain rdf:resource="http://example.org/onto/class/google_scc_folder_custom_module"/>
    <rdfs:range rdf:resource="http://www.w3.org/2001/XMLSchema#string"/>
  </owl:DatatypeProperty>
  <owl:DatatypeProperty rdf:about="http://example.org/onto/prop/google_scc_folder_custom_module_update">
    <rdfs:label>update</rdfs:label>
    <rdfs:domain rdf:resource="http://example.org/onto/class/google_scc_folder_custom_module"/>
    <rdfs:range rdf:resource="http://www.w3.org/2001/XMLSchema#string"/>
  </owl:DatatypeProperty>
</rdf:RDF>
