<?xml version="1.0" encoding="UTF-8"?>
<rdf:RDF
  xmlns:rdf="http://www.w3.org/1999/02/22-rdf-syntax-ns#"
  xmlns:rdfs="http://www.w3.org/2000/01/rdf-schema#"
  xmlns:owl="http://www.w3.org/2002/07/owl#"
  xmlns:xsd="http://www.w3.org/2001/XMLSchema#"
  xml:base="http://example.org/onto/">
  <owl:Class rdf:about="http://example.org/onto/class/google_oracle_database_autonomous_database">
    <rdfs:label>google_oracle_database_autonomous_database</rdfs:label>
    <rdfs:comment>#
#     ***     AUTO GENERATED CODE    ***    Type: MMv1     ***
#
# ----------------------------------------------------------------------------
#
#     This code is generated by Magic Modules using the following:
#
#     Configuration: https:#github.com/GoogleCloudPlatform/magic-modules/tree/main/mmv1/products/oracledatabase/AutonomousDatabase.yaml
#     Template:      https:#github.com/GoogleCloudPlatform/magic-modules/tree/main/mmv1/templates/terraform/resource.html.markdown.tmpl
#
#     DO NOT EDIT this file directly. Any changes made to this file will be
#     overwritten during the next generation cycle.
#
# ----------------------------------------------------------------------------
subcategory: "Oracle Database"
description: |-
  An AutonomousDatabase resource.
---</rdfs:comment>
  </owl:Class>
  <owl:DatatypeProperty rdf:about="http://example.org/onto/prop/google_oracle_database_autonomous_database_admin_password">
    <rdfs:label>admin_password</rdfs:label>
    <rdfs:comment>The password for the default ADMIN user.</rdfs:comment>
    <rdfs:domain rdf:resource="http://example.org/onto/class/google_oracle_database_autonomous_database"/>
    <rdfs:range rdf:resource="http://www.w3.org/2001/XMLSchema#string"/>
  </owl:DatatypeProperty>
  <owl:DatatypeProperty rdf:about="http://example.org/onto/prop/google_oracle_database_autonomous_database_autonomous_database_id">
    <rdfs:label>autonomous_database_id</rdfs:label>
    <rdfs:comment>The ID of the Autonomous Database to create. This value is restricted
to (^[a-z]([a-z0-9-]{0,61}[a-z0-9])?$) and must be a maximum of 63
characters in length. The value must start with a letter and end with
a letter or a number.</rdfs:comment>
    <rdfs:domain rdf:resource="http://example.org/onto/class/google_oracle_database_autonomous_database"/>
    <rdfs:range rdf:resource="http://www.w3.org/2001/XMLSchema#string"/>
  </owl:DatatypeProperty>
  <owl:DatatypeProperty rdf:about="http://example.org/onto/prop/google_oracle_database_autonomous_database_cidr">
    <rdfs:label>cidr</rdfs:label>
    <rdfs:comment>The subnet CIDR range for the Autonmous Database.</rdfs:comment>
    <rdfs:domain rdf:resource="http://example.org/onto/class/google_oracle_database_autonomous_database"/>
    <rdfs:range rdf:resource="http://www.w3.org/2001/XMLSchema#string"/>
  </owl:DatatypeProperty>
  <owl:DatatypeProperty rdf:about="http://example.org/onto/prop/google_oracle_database_autonomous_database_create_time">
    <rdfs:label>create_time</rdfs:label>
    <rdfs:comment>The date and time that the Autonomous Database was created.</rdfs:comment>
    <rdfs:domain rdf:resource="http://example.org/onto/class/google_oracle_database_autonomous_database"/>
    <rdfs:range rdf:resource="http://www.w3.org/2001/XMLSchema#string"/>
  </owl:DatatypeProperty>
  <owl:DatatypeProperty rdf:about="http://example.org/onto/prop/google_oracle_database_autonomous_database_database">
    <rdfs:label>database</rdfs:label>
    <rdfs:comment>The name of the Autonomous Database. The database name must be unique in
the project. The name must begin with a letter and can
contain a maximum of 30 alphanumeric characters.</rdfs:comment>
    <rdfs:domain rdf:resource="http://example.org/onto/class/google_oracle_database_autonomous_database"/>
    <rdfs:range rdf:resource="http://www.w3.org/2001/XMLSchema#string"/>
  </owl:DatatypeProperty>
  <owl:DatatypeProperty rdf:about="http://example.org/onto/prop/google_oracle_database_autonomous_database_deletion_protection">
    <rdfs:label>deletion_protection</rdfs:label>
    <rdfs:comment>Whether or not to allow Terraform to destroy the instance. Unless this field is set to false in Terraform state, a terraform destroy or terraform apply that would delete the instance will fail.</rdfs:comment>
    <rdfs:domain rdf:resource="http://example.org/onto/class/google_oracle_database_autonomous_database"/>
    <rdfs:range rdf:resource="http://www.w3.org/2001/XMLSchema#string"/>
  </owl:DatatypeProperty>
  <owl:DatatypeProperty rdf:about="http://example.org/onto/prop/google_oracle_database_autonomous_database_display_name">
    <rdfs:label>display_name</rdfs:label>
    <rdfs:comment>The display name for the Autonomous Database. The name does not have to
be unique within your project.</rdfs:comment>
    <rdfs:domain rdf:resource="http://example.org/onto/class/google_oracle_database_autonomous_database"/>
    <rdfs:range rdf:resource="http://www.w3.org/2001/XMLSchema#string"/>
  </owl:DatatypeProperty>
  <owl:DatatypeProperty rdf:about="http://example.org/onto/prop/google_oracle_database_autonomous_database_effective_labels">
    <rdfs:label>effective_labels</rdfs:label>
    <rdfs:comment>All of labels (key/value pairs) present on the resource in GCP, including the labels configured through Terraform, other clients and services.</rdfs:comment>
    <rdfs:domain rdf:resource="http://example.org/onto/class/google_oracle_database_autonomous_database"/>
    <rdfs:range rdf:resource="http://www.w3.org/2001/XMLSchema#string"/>
  </owl:DatatypeProperty>
  <owl:DatatypeProperty rdf:about="http://example.org/onto/prop/google_oracle_database_autonomous_database_entitlement_id">
    <rdfs:label>entitlement_id</rdfs:label>
    <rdfs:comment>The ID of the subscription entitlement associated with the Autonomous
Database.</rdfs:comment>
    <rdfs:domain rdf:resource="http://example.org/onto/class/google_oracle_database_autonomous_database"/>
    <rdfs:range rdf:resource="http://www.w3.org/2001/XMLSchema#string"/>
  </owl:DatatypeProperty>
  <owl:DatatypeProperty rdf:about="http://example.org/onto/prop/google_oracle_database_autonomous_database_id">
    <rdfs:label>id</rdfs:label>
    <rdfs:domain rdf:resource="http://example.org/onto/class/google_oracle_database_autonomous_database"/>
    <rdfs:range rdf:resource="http://www.w3.org/2001/XMLSchema#string"/>
  </owl:DatatypeProperty>
  <owl:DatatypeProperty rdf:about="http://example.org/onto/prop/google_oracle_database_autonomous_database_labels">
    <rdfs:label>labels</rdfs:label>
    <rdfs:comment>The labels or tags associated with the Autonomous Database. 

**Note**: This field is non-authoritative, and will only manage the labels present in your configuration.
Please refer to the field 'effective_labels' for all of the labels present on the resource.</rdfs:comment>
    <rdfs:domain rdf:resource="http://example.org/onto/class/google_oracle_database_autonomous_database"/>
    <rdfs:range rdf:resource="http://www.w3.org/2001/XMLSchema#string"/>
  </owl:DatatypeProperty>
  <owl:DatatypeProperty rdf:about="http://example.org/onto/prop/google_oracle_database_autonomous_database_location">
    <rdfs:label>location</rdfs:label>
    <rdfs:comment>Resource ID segment making up resource 'name'. See documentation for resource type 'oracledatabase.googleapis.com/AutonomousDatabaseBackup'.</rdfs:comment>
    <rdfs:domain rdf:resource="http://example.org/onto/class/google_oracle_database_autonomous_database"/>
    <rdfs:range rdf:resource="http://www.w3.org/2001/XMLSchema#string"/>
  </owl:DatatypeProperty>
  <owl:DatatypeProperty rdf:about="http://example.org/onto/prop/google_oracle_database_autonomous_database_name">
    <rdfs:label>name</rdfs:label>
    <rdfs:comment>Identifier. The name of the Autonomous Database resource in the following format:
projects/{project}/locations/{region}/autonomousDatabases/{autonomous_database}</rdfs:comment>
    <rdfs:domain rdf:resource="http://example.org/onto/class/google_oracle_database_autonomous_database"/>
    <rdfs:range rdf:resource="http://www.w3.org/2001/XMLSchema#string"/>
  </owl:DatatypeProperty>
  <owl:DatatypeProperty rdf:about="http://example.org/onto/prop/google_oracle_database_autonomous_database_network">
    <rdfs:label>network</rdfs:label>
    <rdfs:comment>The name of the VPC network used by the Autonomous Database.
Format: projects/{project}/global/networks/{network}</rdfs:comment>
    <rdfs:domain rdf:resource="http://example.org/onto/class/google_oracle_database_autonomous_database"/>
    <rdfs:range rdf:resource="http://www.w3.org/2001/XMLSchema#string"/>
  </owl:DatatypeProperty>
  <owl:DatatypeProperty rdf:about="http://example.org/onto/prop/google_oracle_database_autonomous_database_odb_network">
    <rdfs:label>odb_network</rdfs:label>
    <rdfs:comment>The name of the OdbNetwork associated with the Autonomous Database.
Format:
projects/{project}/locations/{location}/odbNetworks/{odb_network}
It is optional but if specified, this should match the parent ODBNetwork of
the odb_subnet and backup_odb_subnet.</rdfs:comment>
    <rdfs:domain rdf:resource="http://example.org/onto/class/google_oracle_database_autonomous_database"/>
    <rdfs:range rdf:resource="http://www.w3.org/2001/XMLSchema#string"/>
  </owl:DatatypeProperty>
  <owl:DatatypeProperty rdf:about="http://example.org/onto/prop/google_oracle_database_autonomous_database_odb_subnet">
    <rdfs:label>odb_subnet</rdfs:label>
    <rdfs:comment>The name of the OdbSubnet associated with the Autonomous Database for
IP allocation. Format:
projects/{project}/locations/{location}/odbNetworks/{odb_network}/odbSubnets/{odb_subnet}</rdfs:comment>
    <rdfs:domain rdf:resource="http://example.org/onto/class/google_oracle_database_autonomous_database"/>
    <rdfs:range rdf:resource="http://www.w3.org/2001/XMLSchema#string"/>
  </owl:DatatypeProperty>
  <owl:DatatypeProperty rdf:about="http://example.org/onto/prop/google_oracle_database_autonomous_database_project">
    <rdfs:label>project</rdfs:label>
    <rdfs:domain rdf:resource="http://example.org/onto/class/google_oracle_database_autonomous_database"/>
    <rdfs:range rdf:resource="http://www.w3.org/2001/XMLSchema#string"/>
  </owl:DatatypeProperty>
  <owl:DatatypeProperty rdf:about="http://example.org/onto/prop/google_oracle_database_autonomous_database_terraform_labels">
    <rdfs:label>terraform_labels</rdfs:label>
    <rdfs:comment>The combination of labels configured directly on the resource
 and default labels configured on the provider.</rdfs:comment>
    <rdfs:domain rdf:resource="http://example.org/onto/class/google_oracle_database_autonomous_database"/>
    <rdfs:range rdf:resource="http://www.w3.org/2001/XMLSchema#string"/>
  </owl:DatatypeProperty>
  <owl:DatatypeProperty rdf:about="http://example.org/onto/prop/google_oracle_database_autonomous_database_actual_used_data_storage_size_tb">
    <rdfs:label>actual_used_data_storage_size_tb</rdfs:label>
    <rdfs:comment>The amount of storage currently being used for user and system data, in
terabytes.</rdfs:comment>
    <rdfs:domain rdf:resource="http://example.org/onto/class/google_oracle_database_autonomous_database"/>
    <rdfs:range rdf:resource="http://www.w3.org/2001/XMLSchema#string"/>
  </owl:DatatypeProperty>
  <owl:DatatypeProperty rdf:about="http://example.org/onto/prop/google_oracle_database_autonomous_database_allocated_storage_size_tb">
    <rdfs:label>allocated_storage_size_tb</rdfs:label>
    <rdfs:comment>The amount of storage currently allocated for the database tables and
billed for, rounded up in terabytes.</rdfs:comment>
    <rdfs:domain rdf:resource="http://example.org/onto/class/google_oracle_database_autonomous_database"/>
    <rdfs:range rdf:resource="http://www.w3.org/2001/XMLSchema#string"/>
  </owl:DatatypeProperty>
  <owl:DatatypeProperty rdf:about="http://example.org/onto/prop/google_oracle_database_autonomous_database_apex_details">
    <rdfs:label>apex_details</rdfs:label>
    <rdfs:comment>Oracle APEX Application Development.
https://docs.oracle.com/en-us/iaas/api/#/en/database/20160918/datatypes/AutonomousDatabaseApex</rdfs:comment>
    <rdfs:domain rdf:resource="http://example.org/onto/class/google_oracle_database_autonomous_database"/>
    <rdfs:range rdf:resource="http://www.w3.org/2001/XMLSchema#string"/>
  </owl:DatatypeProperty>
  <owl:DatatypeProperty rdf:about="http://example.org/onto/prop/google_oracle_database_autonomous_database_are_primary_allowlisted_ips_used">
    <rdfs:label>are_primary_allowlisted_ips_used</rdfs:label>
    <rdfs:comment>This field indicates the status of Data Guard and Access control for the
Autonomous Database. The field's value is null if Data Guard is disabled
or Access Control is disabled. The field's value is TRUE if both Data Guard
and Access Control are enabled, and the Autonomous Database is using
primary IP access control list (ACL) for standby. The field's value is
FALSE if both Data Guard and Access Control are enabled, and the Autonomous
Database is using a different IP access control list (ACL) for standby
compared to primary.</rdfs:comment>
    <rdfs:domain rdf:resource="http://example.org/onto/class/google_oracle_database_autonomous_database"/>
    <rdfs:range rdf:resource="http://www.w3.org/2001/XMLSchema#string"/>
  </owl:DatatypeProperty>
  <owl:DatatypeProperty rdf:about="http://example.org/onto/prop/google_oracle_database_autonomous_database_autonomous_container_database_id">
    <rdfs:label>autonomous_container_database_id</rdfs:label>
    <rdfs:comment>The Autonomous Container Database OCID.</rdfs:comment>
    <rdfs:domain rdf:resource="http://example.org/onto/class/google_oracle_database_autonomous_database"/>
    <rdfs:range rdf:resource="http://www.w3.org/2001/XMLSchema#string"/>
  </owl:DatatypeProperty>
  <owl:DatatypeProperty rdf:about="http://example.org/onto/prop/google_oracle_database_autonomous_database_available_upgrade_versions">
    <rdfs:label>available_upgrade_versions</rdfs:label>
    <rdfs:comment>The list of available Oracle Database upgrade versions for an Autonomous
Database.</rdfs:comment>
    <rdfs:domain rdf:resource="http://example.org/onto/class/google_oracle_database_autonomous_database"/>
    <rdfs:range rdf:resource="http://www.w3.org/2001/XMLSchema#string"/>
  </owl:DatatypeProperty>
  <owl:DatatypeProperty rdf:about="http://example.org/onto/prop/google_oracle_database_autonomous_database_backup_retention_period_days">
    <rdfs:label>backup_retention_period_days</rdfs:label>
    <rdfs:comment>The retention period for the Autonomous Database. This field is specified
in days, can range from 1 day to 60 days, and has a default value of
60 days.</rdfs:comment>
    <rdfs:domain rdf:resource="http://example.org/onto/class/google_oracle_database_autonomous_database"/>
    <rdfs:range rdf:resource="http://www.w3.org/2001/XMLSchema#string"/>
  </owl:DatatypeProperty>
  <owl:DatatypeProperty rdf:about="http://example.org/onto/prop/google_oracle_database_autonomous_database_character_set">
    <rdfs:label>character_set</rdfs:label>
    <rdfs:comment>The character set for the Autonomous Database. The default is AL32UTF8.</rdfs:comment>
    <rdfs:domain rdf:resource="http://example.org/onto/class/google_oracle_database_autonomous_database"/>
    <rdfs:range rdf:resource="http://www.w3.org/2001/XMLSchema#string"/>
  </owl:DatatypeProperty>
  <owl:DatatypeProperty rdf:about="http://example.org/onto/prop/google_oracle_database_autonomous_database_compute_count">
    <rdfs:label>compute_count</rdfs:label>
    <rdfs:comment>The number of compute servers for the Autonomous Database.</rdfs:comment>
    <rdfs:domain rdf:resource="http://example.org/onto/class/google_oracle_database_autonomous_database"/>
    <rdfs:range rdf:resource="http://www.w3.org/2001/XMLSchema#string"/>
  </owl:DatatypeProperty>
  <owl:DatatypeProperty rdf:about="http://example.org/onto/prop/google_oracle_database_autonomous_database_connection_strings">
    <rdfs:label>connection_strings</rdfs:label>
    <rdfs:comment>The connection string used to connect to the Autonomous Database.
https://docs.oracle.com/en-us/iaas/api/#/en/database/20160918/datatypes/AutonomousDatabaseConnectionStrings</rdfs:comment>
    <rdfs:domain rdf:resource="http://example.org/onto/class/google_oracle_database_autonomous_database"/>
    <rdfs:range rdf:resource="http://www.w3.org/2001/XMLSchema#string"/>
  </owl:DatatypeProperty>
  <owl:DatatypeProperty rdf:about="http://example.org/onto/prop/google_oracle_database_autonomous_database_connection_urls">
    <rdfs:label>connection_urls</rdfs:label>
    <rdfs:comment>The URLs for accessing Oracle Application Express (APEX) and SQL Developer
Web with a browser from a Compute instance.
https://docs.oracle.com/en-us/iaas/api/#/en/database/20160918/datatypes/AutonomousDatabaseConnectionUrls</rdfs:comment>
    <rdfs:domain rdf:resource="http://example.org/onto/class/google_oracle_database_autonomous_database"/>
    <rdfs:range rdf:resource="http://www.w3.org/2001/XMLSchema#string"/>
  </owl:DatatypeProperty>
  <owl:DatatypeProperty rdf:about="http://example.org/onto/prop/google_oracle_database_autonomous_database_data_safe_state">
    <rdfs:label>data_safe_state</rdfs:label>
    <rdfs:comment>The current state of the Data Safe registration for the
Autonomous Database. 
 Possible values:
 DATA_SAFE_STATE_UNSPECIFIED
REGISTERING
REGISTERED
DEREGISTERING
NOT_REGISTERED
FAILED</rdfs:comment>
    <rdfs:domain rdf:resource="http://example.org/onto/class/google_oracle_database_autonomous_database"/>
    <rdfs:range rdf:resource="http://www.w3.org/2001/XMLSchema#string"/>
  </owl:DatatypeProperty>
  <owl:DatatypeProperty rdf:about="http://example.org/onto/prop/google_oracle_database_autonomous_database_data_storage_size_gb">
    <rdfs:label>data_storage_size_gb</rdfs:label>
    <rdfs:comment>The size of the data stored in the database, in gigabytes.</rdfs:comment>
    <rdfs:domain rdf:resource="http://example.org/onto/class/google_oracle_database_autonomous_database"/>
    <rdfs:range rdf:resource="http://www.w3.org/2001/XMLSchema#string"/>
  </owl:DatatypeProperty>
  <owl:DatatypeProperty rdf:about="http://example.org/onto/prop/google_oracle_database_autonomous_database_data_storage_size_tb">
    <rdfs:label>data_storage_size_tb</rdfs:label>
    <rdfs:comment>The size of the data stored in the database, in terabytes.</rdfs:comment>
    <rdfs:domain rdf:resource="http://example.org/onto/class/google_oracle_database_autonomous_database"/>
    <rdfs:range rdf:resource="http://www.w3.org/2001/XMLSchema#string"/>
  </owl:DatatypeProperty>
  <owl:DatatypeProperty rdf:about="http://example.org/onto/prop/google_oracle_database_autonomous_database_database_management_state">
    <rdfs:label>database_management_state</rdfs:label>
    <rdfs:comment>The current state of database management for the Autonomous Database. 
 Possible values:
 DATABASE_MANAGEMENT_STATE_UNSPECIFIED
ENABLING
ENABLED
DISABLING
NOT_ENABLED
FAILED_ENABLING
FAILED_DISABLING</rdfs:comment>
    <rdfs:domain rdf:resource="http://example.org/onto/class/google_oracle_database_autonomous_database"/>
    <rdfs:range rdf:resource="http://www.w3.org/2001/XMLSchema#string"/>
  </owl:DatatypeProperty>
  <owl:DatatypeProperty rdf:about="http://example.org/onto/prop/google_oracle_database_autonomous_database_db_edition">
    <rdfs:label>db_edition</rdfs:label>
    <rdfs:comment>The edition of the Autonomous Databases. 
 Possible values:
 DATABASE_EDITION_UNSPECIFIED
STANDARD_EDITION
ENTERPRISE_EDITION</rdfs:comment>
    <rdfs:domain rdf:resource="http://example.org/onto/class/google_oracle_database_autonomous_database"/>
    <rdfs:range rdf:resource="http://www.w3.org/2001/XMLSchema#string"/>
  </owl:DatatypeProperty>
  <owl:DatatypeProperty rdf:about="http://example.org/onto/prop/google_oracle_database_autonomous_database_db_version">
    <rdfs:label>db_version</rdfs:label>
    <rdfs:comment>The Oracle Database version for the Autonomous Database.</rdfs:comment>
    <rdfs:domain rdf:resource="http://example.org/onto/class/google_oracle_database_autonomous_database"/>
    <rdfs:range rdf:resource="http://www.w3.org/2001/XMLSchema#string"/>
  </owl:DatatypeProperty>
  <owl:DatatypeProperty rdf:about="http://example.org/onto/prop/google_oracle_database_autonomous_database_db_workload">
    <rdfs:label>db_workload</rdfs:label>
    <rdfs:comment>Possible values:
 DB_WORKLOAD_UNSPECIFIED
OLTP
DW
AJD
APEX</rdfs:comment>
    <rdfs:domain rdf:resource="http://example.org/onto/class/google_oracle_database_autonomous_database"/>
    <rdfs:range rdf:resource="http://www.w3.org/2001/XMLSchema#string"/>
  </owl:DatatypeProperty>
  <owl:DatatypeProperty rdf:about="http://example.org/onto/prop/google_oracle_database_autonomous_database_failed_data_recovery_duration">
    <rdfs:label>failed_data_recovery_duration</rdfs:label>
    <rdfs:comment>This field indicates the number of seconds of data loss during a Data
Guard failover.</rdfs:comment>
    <rdfs:domain rdf:resource="http://example.org/onto/class/google_oracle_database_autonomous_database"/>
    <rdfs:range rdf:resource="http://www.w3.org/2001/XMLSchema#string"/>
  </owl:DatatypeProperty>
  <owl:DatatypeProperty rdf:about="http://example.org/onto/prop/google_oracle_database_autonomous_database_is_auto_scaling_enabled">
    <rdfs:label>is_auto_scaling_enabled</rdfs:label>
    <rdfs:comment>This field indicates if auto scaling is enabled for the Autonomous Database
CPU core count.</rdfs:comment>
    <rdfs:domain rdf:resource="http://example.org/onto/class/google_oracle_database_autonomous_database"/>
    <rdfs:range rdf:resource="http://www.w3.org/2001/XMLSchema#string"/>
  </owl:DatatypeProperty>
  <owl:DatatypeProperty rdf:about="http://example.org/onto/prop/google_oracle_database_autonomous_database_is_local_data_guard_enabled">
    <rdfs:label>is_local_data_guard_enabled</rdfs:label>
    <rdfs:comment>This field indicates whether the Autonomous Database has local (in-region)
Data Guard enabled.</rdfs:comment>
    <rdfs:domain rdf:resource="http://example.org/onto/class/google_oracle_database_autonomous_database"/>
    <rdfs:range rdf:resource="http://www.w3.org/2001/XMLSchema#string"/>
  </owl:DatatypeProperty>
  <owl:DatatypeProperty rdf:about="http://example.org/onto/prop/google_oracle_database_autonomous_database_is_storage_auto_scaling_enabled">
    <rdfs:label>is_storage_auto_scaling_enabled</rdfs:label>
    <rdfs:comment>This field indicates if auto scaling is enabled for the Autonomous Database
storage.</rdfs:comment>
    <rdfs:domain rdf:resource="http://example.org/onto/class/google_oracle_database_autonomous_database"/>
    <rdfs:range rdf:resource="http://www.w3.org/2001/XMLSchema#string"/>
  </owl:DatatypeProperty>
  <owl:DatatypeProperty rdf:about="http://example.org/onto/prop/google_oracle_database_autonomous_database_license_type">
    <rdfs:label>license_type</rdfs:label>
    <rdfs:comment>The license type used for the Autonomous Database. 
 Possible values:
 LICENSE_TYPE_UNSPECIFIED
LICENSE_INCLUDED
BRING_YOUR_OWN_LICENSE</rdfs:comment>
    <rdfs:domain rdf:resource="http://example.org/onto/class/google_oracle_database_autonomous_database"/>
    <rdfs:range rdf:resource="http://www.w3.org/2001/XMLSchema#string"/>
  </owl:DatatypeProperty>
  <owl:DatatypeProperty rdf:about="http://example.org/onto/prop/google_oracle_database_autonomous_database_lifecycle_details">
    <rdfs:label>lifecycle_details</rdfs:label>
    <rdfs:comment>The details of the current lifestyle state of the Autonomous Database.</rdfs:comment>
    <rdfs:domain rdf:resource="http://example.org/onto/class/google_oracle_database_autonomous_database"/>
    <rdfs:range rdf:resource="http://www.w3.org/2001/XMLSchema#string"/>
  </owl:DatatypeProperty>
  <owl:DatatypeProperty rdf:about="http://example.org/onto/prop/google_oracle_database_autonomous_database_local_adg_auto_failover_max_data_loss_limit">
    <rdfs:label>local_adg_auto_failover_max_data_loss_limit</rdfs:label>
    <rdfs:comment>This field indicates the maximum data loss limit for an Autonomous
Database, in seconds.</rdfs:comment>
    <rdfs:domain rdf:resource="http://example.org/onto/class/google_oracle_database_autonomous_database"/>
    <rdfs:range rdf:resource="http://www.w3.org/2001/XMLSchema#string"/>
  </owl:DatatypeProperty>
  <owl:DatatypeProperty rdf:about="http://example.org/onto/prop/google_oracle_database_autonomous_database_local_disaster_recovery_type">
    <rdfs:label>local_disaster_recovery_type</rdfs:label>
    <rdfs:comment>This field indicates the local disaster recovery (DR) type of an
Autonomous Database. 
 Possible values:
 LOCAL_DISASTER_RECOVERY_TYPE_UNSPECIFIED
ADG
BACKUP_BASED</rdfs:comment>
    <rdfs:domain rdf:resource="http://example.org/onto/class/google_oracle_database_autonomous_database"/>
    <rdfs:range rdf:resource="http://www.w3.org/2001/XMLSchema#string"/>
  </owl:DatatypeProperty>
  <owl:DatatypeProperty rdf:about="http://example.org/onto/prop/google_oracle_database_autonomous_database_local_standby_db">
    <rdfs:label>local_standby_db</rdfs:label>
    <rdfs:comment>Autonomous Data Guard standby database details.
https://docs.oracle.com/en-us/iaas/api/#/en/database/20160918/datatypes/AutonomousDatabaseStandbySummary</rdfs:comment>
    <rdfs:domain rdf:resource="http://example.org/onto/class/google_oracle_database_autonomous_database"/>
    <rdfs:range rdf:resource="http://www.w3.org/2001/XMLSchema#string"/>
  </owl:DatatypeProperty>
  <owl:DatatypeProperty rdf:about="http://example.org/onto/prop/google_oracle_database_autonomous_database_maintenance_begin_time">
    <rdfs:label>maintenance_begin_time</rdfs:label>
    <rdfs:comment>The date and time when maintenance will begin.</rdfs:comment>
    <rdfs:domain rdf:resource="http://example.org/onto/class/google_oracle_database_autonomous_database"/>
    <rdfs:range rdf:resource="http://www.w3.org/2001/XMLSchema#string"/>
  </owl:DatatypeProperty>
  <owl:DatatypeProperty rdf:about="http://example.org/onto/prop/google_oracle_database_autonomous_database_maintenance_end_time">
    <rdfs:label>maintenance_end_time</rdfs:label>
    <rdfs:comment>The date and time when maintenance will end.</rdfs:comment>
    <rdfs:domain rdf:resource="http://example.org/onto/class/google_oracle_database_autonomous_database"/>
    <rdfs:range rdf:resource="http://www.w3.org/2001/XMLSchema#string"/>
  </owl:DatatypeProperty>
  <owl:DatatypeProperty rdf:about="http://example.org/onto/prop/google_oracle_database_autonomous_database_maintenance_schedule_type">
    <rdfs:label>maintenance_schedule_type</rdfs:label>
    <rdfs:comment>The maintenance schedule of the Autonomous Database. 
 Possible values:
 MAINTENANCE_SCHEDULE_TYPE_UNSPECIFIED
EARLY
REGULAR</rdfs:comment>
    <rdfs:domain rdf:resource="http://example.org/onto/class/google_oracle_database_autonomous_database"/>
    <rdfs:range rdf:resource="http://www.w3.org/2001/XMLSchema#string"/>
  </owl:DatatypeProperty>
  <owl:DatatypeProperty rdf:about="http://example.org/onto/prop/google_oracle_database_autonomous_database_memory_per_oracle_compute_unit_gbs">
    <rdfs:label>memory_per_oracle_compute_unit_gbs</rdfs:label>
    <rdfs:comment>The amount of memory enabled per ECPU, in gigabytes.</rdfs:comment>
    <rdfs:domain rdf:resource="http://example.org/onto/class/google_oracle_database_autonomous_database"/>
    <rdfs:range rdf:resource="http://www.w3.org/2001/XMLSchema#string"/>
  </owl:DatatypeProperty>
  <owl:DatatypeProperty rdf:about="http://example.org/onto/prop/google_oracle_database_autonomous_database_memory_table_gbs">
    <rdfs:label>memory_table_gbs</rdfs:label>
    <rdfs:comment>The memory assigned to in-memory tables in an Autonomous Database.</rdfs:comment>
    <rdfs:domain rdf:resource="http://example.org/onto/class/google_oracle_database_autonomous_database"/>
    <rdfs:range rdf:resource="http://www.w3.org/2001/XMLSchema#string"/>
  </owl:DatatypeProperty>
  <owl:DatatypeProperty rdf:about="http://example.org/onto/prop/google_oracle_database_autonomous_database_mtls_connection_required">
    <rdfs:label>mtls_connection_required</rdfs:label>
    <rdfs:comment>This field specifies if the Autonomous Database requires mTLS connections.</rdfs:comment>
    <rdfs:domain rdf:resource="http://example.org/onto/class/google_oracle_database_autonomous_database"/>
    <rdfs:range rdf:resource="http://www.w3.org/2001/XMLSchema#string"/>
  </owl:DatatypeProperty>
  <owl:DatatypeProperty rdf:about="http://example.org/onto/prop/google_oracle_database_autonomous_database_n_character_set">
    <rdfs:label>n_character_set</rdfs:label>
    <rdfs:comment>The national character set for the Autonomous Database. The default is
AL16UTF16.</rdfs:comment>
    <rdfs:domain rdf:resource="http://example.org/onto/class/google_oracle_database_autonomous_database"/>
    <rdfs:range rdf:resource="http://www.w3.org/2001/XMLSchema#string"/>
  </owl:DatatypeProperty>
  <owl:DatatypeProperty rdf:about="http://example.org/onto/prop/google_oracle_database_autonomous_database_next_long_term_backup_time">
    <rdfs:label>next_long_term_backup_time</rdfs:label>
    <rdfs:comment>The long term backup schedule of the Autonomous Database.</rdfs:comment>
    <rdfs:domain rdf:resource="http://example.org/onto/class/google_oracle_database_autonomous_database"/>
    <rdfs:range rdf:resource="http://www.w3.org/2001/XMLSchema#string"/>
  </owl:DatatypeProperty>
  <owl:DatatypeProperty rdf:about="http://example.org/onto/prop/google_oracle_database_autonomous_database_oci_url">
    <rdfs:label>oci_url</rdfs:label>
    <rdfs:comment>The Oracle Cloud Infrastructure link for the Autonomous Database.</rdfs:comment>
    <rdfs:domain rdf:resource="http://example.org/onto/class/google_oracle_database_autonomous_database"/>
    <rdfs:range rdf:resource="http://www.w3.org/2001/XMLSchema#string"/>
  </owl:DatatypeProperty>
  <owl:DatatypeProperty rdf:about="http://example.org/onto/prop/google_oracle_database_autonomous_database_ocid">
    <rdfs:label>ocid</rdfs:label>
    <rdfs:comment>OCID of the Autonomous Database.
https://docs.oracle.com/en-us/iaas/Content/General/Concepts/identifiers.htm#Oracle</rdfs:comment>
    <rdfs:domain rdf:resource="http://example.org/onto/class/google_oracle_database_autonomous_database"/>
    <rdfs:range rdf:resource="http://www.w3.org/2001/XMLSchema#string"/>
  </owl:DatatypeProperty>
  <owl:DatatypeProperty rdf:about="http://example.org/onto/prop/google_oracle_database_autonomous_database_open_mode">
    <rdfs:label>open_mode</rdfs:label>
    <rdfs:comment>This field indicates the current mode of the Autonomous Database. 
 Possible values:
 OPEN_MODE_UNSPECIFIED
READ_ONLY
READ_WRITE</rdfs:comment>
    <rdfs:domain rdf:resource="http://example.org/onto/class/google_oracle_database_autonomous_database"/>
    <rdfs:range rdf:resource="http://www.w3.org/2001/XMLSchema#string"/>
  </owl:DatatypeProperty>
  <owl:DatatypeProperty rdf:about="http://example.org/onto/prop/google_oracle_database_autonomous_database_operations_insights_state">
    <rdfs:label>operations_insights_state</rdfs:label>
    <rdfs:comment>Possible values:
 OPERATIONS_INSIGHTS_STATE_UNSPECIFIED
ENABLING
ENABLED
DISABLING
NOT_ENABLED
FAILED_ENABLING
FAILED_DISABLING</rdfs:comment>
    <rdfs:domain rdf:resource="http://example.org/onto/class/google_oracle_database_autonomous_database"/>
    <rdfs:range rdf:resource="http://www.w3.org/2001/XMLSchema#string"/>
  </owl:DatatypeProperty>
  <owl:DatatypeProperty rdf:about="http://example.org/onto/prop/google_oracle_database_autonomous_database_peer_db_ids">
    <rdfs:label>peer_db_ids</rdfs:label>
    <rdfs:comment>The list of OCIDs of standby databases located in Autonomous Data Guard
remote regions that are associated with the source database.</rdfs:comment>
    <rdfs:domain rdf:resource="http://example.org/onto/class/google_oracle_database_autonomous_database"/>
    <rdfs:range rdf:resource="http://www.w3.org/2001/XMLSchema#string"/>
  </owl:DatatypeProperty>
  <owl:DatatypeProperty rdf:about="http://example.org/onto/prop/google_oracle_database_autonomous_database_permission_level">
    <rdfs:label>permission_level</rdfs:label>
    <rdfs:comment>The permission level of the Autonomous Database. 
 Possible values:
 PERMISSION_LEVEL_UNSPECIFIED
RESTRICTED
UNRESTRICTED</rdfs:comment>
    <rdfs:domain rdf:resource="http://example.org/onto/class/google_oracle_database_autonomous_database"/>
    <rdfs:range rdf:resource="http://www.w3.org/2001/XMLSchema#string"/>
  </owl:DatatypeProperty>
  <owl:DatatypeProperty rdf:about="http://example.org/onto/prop/google_oracle_database_autonomous_database_private_endpoint">
    <rdfs:label>private_endpoint</rdfs:label>
    <rdfs:comment>The private endpoint for the Autonomous Database.</rdfs:comment>
    <rdfs:domain rdf:resource="http://example.org/onto/class/google_oracle_database_autonomous_database"/>
    <rdfs:range rdf:resource="http://www.w3.org/2001/XMLSchema#string"/>
  </owl:DatatypeProperty>
  <owl:DatatypeProperty rdf:about="http://example.org/onto/prop/google_oracle_database_autonomous_database_private_endpoint_ip">
    <rdfs:label>private_endpoint_ip</rdfs:label>
    <rdfs:comment>The private endpoint IP address for the Autonomous Database.</rdfs:comment>
    <rdfs:domain rdf:resource="http://example.org/onto/class/google_oracle_database_autonomous_database"/>
    <rdfs:range rdf:resource="http://www.w3.org/2001/XMLSchema#string"/>
  </owl:DatatypeProperty>
  <owl:DatatypeProperty rdf:about="http://example.org/onto/prop/google_oracle_database_autonomous_database_private_endpoint_label">
    <rdfs:label>private_endpoint_label</rdfs:label>
    <rdfs:comment>The private endpoint label for the Autonomous Database.</rdfs:comment>
    <rdfs:domain rdf:resource="http://example.org/onto/class/google_oracle_database_autonomous_database"/>
    <rdfs:range rdf:resource="http://www.w3.org/2001/XMLSchema#string"/>
  </owl:DatatypeProperty>
  <owl:DatatypeProperty rdf:about="http://example.org/onto/prop/google_oracle_database_autonomous_database_refreshable_mode">
    <rdfs:label>refreshable_mode</rdfs:label>
    <rdfs:comment>The refresh mode of the cloned Autonomous Database. 
 Possible values:
 REFRESHABLE_MODE_UNSPECIFIED
AUTOMATIC
MANUAL</rdfs:comment>
    <rdfs:domain rdf:resource="http://example.org/onto/class/google_oracle_database_autonomous_database"/>
    <rdfs:range rdf:resource="http://www.w3.org/2001/XMLSchema#string"/>
  </owl:DatatypeProperty>
  <owl:DatatypeProperty rdf:about="http://example.org/onto/prop/google_oracle_database_autonomous_database_refreshable_state">
    <rdfs:label>refreshable_state</rdfs:label>
    <rdfs:comment>The refresh State of the clone. 
 Possible values:
 REFRESHABLE_STATE_UNSPECIFIED
REFRESHING
NOT_REFRESHING</rdfs:comment>
    <rdfs:domain rdf:resource="http://example.org/onto/class/google_oracle_database_autonomous_database"/>
    <rdfs:range rdf:resource="http://www.w3.org/2001/XMLSchema#string"/>
  </owl:DatatypeProperty>
  <owl:DatatypeProperty rdf:about="http://example.org/onto/prop/google_oracle_database_autonomous_database_role">
    <rdfs:label>role</rdfs:label>
    <rdfs:comment>The Data Guard role of the Autonomous Database. 
 Possible values:
 ROLE_UNSPECIFIED
PRIMARY
STANDBY
DISABLED_STANDBY
BACKUP_COPY
SNAPSHOT_STANDBY</rdfs:comment>
    <rdfs:domain rdf:resource="http://example.org/onto/class/google_oracle_database_autonomous_database"/>
    <rdfs:range rdf:resource="http://www.w3.org/2001/XMLSchema#string"/>
  </owl:DatatypeProperty>
  <owl:DatatypeProperty rdf:about="http://example.org/onto/prop/google_oracle_database_autonomous_database_scheduled_operation_details">
    <rdfs:label>scheduled_operation_details</rdfs:label>
    <rdfs:comment>The list and details of the scheduled operations of the Autonomous
Database.</rdfs:comment>
    <rdfs:domain rdf:resource="http://example.org/onto/class/google_oracle_database_autonomous_database"/>
    <rdfs:range rdf:resource="http://www.w3.org/2001/XMLSchema#string"/>
  </owl:DatatypeProperty>
  <owl:DatatypeProperty rdf:about="http://example.org/onto/prop/google_oracle_database_autonomous_database_sql_web_developer_url">
    <rdfs:label>sql_web_developer_url</rdfs:label>
    <rdfs:comment>The SQL Web Developer URL for the Autonomous Database.</rdfs:comment>
    <rdfs:domain rdf:resource="http://example.org/onto/class/google_oracle_database_autonomous_database"/>
    <rdfs:range rdf:resource="http://www.w3.org/2001/XMLSchema#string"/>
  </owl:DatatypeProperty>
  <owl:DatatypeProperty rdf:about="http://example.org/onto/prop/google_oracle_database_autonomous_database_state">
    <rdfs:label>state</rdfs:label>
    <rdfs:comment>Possible values:
 STATE_UNSPECIFIED
PROVISIONING
AVAILABLE
STOPPING
STOPPED
STARTING
TERMINATING
TERMINATED
UNAVAILABLE
RESTORE_IN_PROGRESS
RESTORE_FAILED
BACKUP_IN_PROGRESS
SCALE_IN_PROGRESS
AVAILABLE_NEEDS_ATTENTION
UPDATING
MAINTENANCE_IN_PROGRESS
RESTARTING
RECREATING
ROLE_CHANGE_IN_PROGRESS
UPGRADING
INACCESSIBLE
STANDBY</rdfs:comment>
    <rdfs:domain rdf:resource="http://example.org/onto/class/google_oracle_database_autonomous_database"/>
    <rdfs:range rdf:resource="http://www.w3.org/2001/XMLSchema#string"/>
  </owl:DatatypeProperty>
  <owl:DatatypeProperty rdf:about="http://example.org/onto/prop/google_oracle_database_autonomous_database_supported_clone_regions">
    <rdfs:label>supported_clone_regions</rdfs:label>
    <rdfs:comment>The list of available regions that can be used to create a clone for the
Autonomous Database.</rdfs:comment>
    <rdfs:domain rdf:resource="http://example.org/onto/class/google_oracle_database_autonomous_database"/>
    <rdfs:range rdf:resource="http://www.w3.org/2001/XMLSchema#string"/>
  </owl:DatatypeProperty>
  <owl:DatatypeProperty rdf:about="http://example.org/onto/prop/google_oracle_database_autonomous_database_total_auto_backup_storage_size_gbs">
    <rdfs:label>total_auto_backup_storage_size_gbs</rdfs:label>
    <rdfs:comment>The storage space used by automatic backups of Autonomous Database, in
gigabytes.</rdfs:comment>
    <rdfs:domain rdf:resource="http://example.org/onto/class/google_oracle_database_autonomous_database"/>
    <rdfs:range rdf:resource="http://www.w3.org/2001/XMLSchema#string"/>
  </owl:DatatypeProperty>
  <owl:DatatypeProperty rdf:about="http://example.org/onto/prop/google_oracle_database_autonomous_database_used_data_storage_size_tbs">
    <rdfs:label>used_data_storage_size_tbs</rdfs:label>
    <rdfs:comment>The storage space used by Autonomous Database, in gigabytes.</rdfs:comment>
    <rdfs:domain rdf:resource="http://example.org/onto/class/google_oracle_database_autonomous_database"/>
    <rdfs:range rdf:resource="http://www.w3.org/2001/XMLSchema#string"/>
  </owl:DatatypeProperty>
  <owl:DatatypeProperty rdf:about="http://example.org/onto/prop/google_oracle_database_autonomous_database_email">
    <rdfs:label>email</rdfs:label>
    <rdfs:comment>The email address used by Oracle to send notifications regarding databases
and infrastructure.</rdfs:comment>
    <rdfs:domain rdf:resource="http://example.org/onto/class/google_oracle_database_autonomous_database"/>
    <rdfs:range rdf:resource="http://www.w3.org/2001/XMLSchema#string"/>
  </owl:DatatypeProperty>
  <owl:DatatypeProperty rdf:about="http://example.org/onto/prop/google_oracle_database_autonomous_database_create">
    <rdfs:label>create</rdfs:label>
    <rdfs:domain rdf:resource="http://example.org/onto/class/google_oracle_database_autonomous_database"/>
    <rdfs:range rdf:resource="http://www.w3.org/2001/XMLSchema#string"/>
  </owl:DatatypeProperty>
  <owl:DatatypeProperty rdf:about="http://example.org/onto/prop/google_oracle_database_autonomous_database_delete">
    <rdfs:label>delete</rdfs:label>
    <rdfs:domain rdf:resource="http://example.org/onto/class/google_oracle_database_autonomous_database"/>
    <rdfs:range rdf:resource="http://www.w3.org/2001/XMLSchema#string"/>
  </owl:DatatypeProperty>
  <owl:DatatypeProperty rdf:about="http://example.org/onto/prop/google_oracle_database_autonomous_database_update">
    <rdfs:label>update</rdfs:label>
    <rdfs:domain rdf:resource="http://example.org/onto/class/google_oracle_database_autonomous_database"/>
    <rdfs:range rdf:resource="http://www.w3.org/2001/XMLSchema#string"/>
  </owl:DatatypeProperty>
</rdf:RDF>
