<?xml version="1.0" encoding="UTF-8"?>
<rdf:RDF
  xmlns:rdf="http://www.w3.org/1999/02/22-rdf-syntax-ns#"
  xmlns:rdfs="http://www.w3.org/2000/01/rdf-schema#"
  xmlns:owl="http://www.w3.org/2002/07/owl#"
  xmlns:xsd="http://www.w3.org/2001/XMLSchema#"
  xml:base="http://example.org/onto/">
  <owl:Class rdf:about="http://example.org/onto/class/google_compute_instance_from_template">
    <rdfs:label>google_compute_instance_from_template</rdfs:label>
    <rdfs:comment>#
#     ***     AUTO GENERATED CODE    ***    Type: Handwritten     ***
#
# ----------------------------------------------------------------------------
#
#     This code is generated by Magic Modules using the following:
#
#     Source file: https://github.com/GoogleCloudPlatform/magic-modules/tree/main/mmv1/third_party/terraform/website/docs/r/compute_instance_from_template.html.markdown
#
#     DO NOT EDIT this file directly. Any changes made to this file will be
#     overwritten during the next generation cycle.
#
# ----------------------------------------------------------------------------
subcategory: "Compute Engine"
description: |-
  Manages a VM instance resource within GCE.
---</rdfs:comment>
  </owl:Class>
  <owl:DatatypeProperty rdf:about="http://example.org/onto/prop/google_compute_instance_from_template_allow_stopping_for_update">
    <rdfs:label>allow_stopping_for_update</rdfs:label>
    <rdfs:comment>If true, allows Terraform to stop the instance to update its properties. If you try to update a property that requires stopping the instance without setting this field, the update will fail.</rdfs:comment>
    <rdfs:domain rdf:resource="http://example.org/onto/class/google_compute_instance_from_template"/>
    <rdfs:range rdf:resource="http://www.w3.org/2001/XMLSchema#string"/>
  </owl:DatatypeProperty>
  <owl:DatatypeProperty rdf:about="http://example.org/onto/prop/google_compute_instance_from_template_can_ip_forward">
    <rdfs:label>can_ip_forward</rdfs:label>
    <rdfs:comment>Whether sending and receiving of packets with non-matching source or destination IPs is allowed.</rdfs:comment>
    <rdfs:domain rdf:resource="http://example.org/onto/class/google_compute_instance_from_template"/>
    <rdfs:range rdf:resource="http://www.w3.org/2001/XMLSchema#string"/>
  </owl:DatatypeProperty>
  <owl:DatatypeProperty rdf:about="http://example.org/onto/prop/google_compute_instance_from_template_cpu_platform">
    <rdfs:label>cpu_platform</rdfs:label>
    <rdfs:comment>The CPU platform used by this instance.</rdfs:comment>
    <rdfs:domain rdf:resource="http://example.org/onto/class/google_compute_instance_from_template"/>
    <rdfs:range rdf:resource="http://www.w3.org/2001/XMLSchema#string"/>
  </owl:DatatypeProperty>
  <owl:DatatypeProperty rdf:about="http://example.org/onto/prop/google_compute_instance_from_template_creation_timestamp">
    <rdfs:label>creation_timestamp</rdfs:label>
    <rdfs:comment>Creation timestamp in RFC3339 text format.</rdfs:comment>
    <rdfs:domain rdf:resource="http://example.org/onto/class/google_compute_instance_from_template"/>
    <rdfs:range rdf:resource="http://www.w3.org/2001/XMLSchema#string"/>
  </owl:DatatypeProperty>
  <owl:DatatypeProperty rdf:about="http://example.org/onto/prop/google_compute_instance_from_template_current_status">
    <rdfs:label>current_status</rdfs:label>
    <rdfs:comment>Current status of the instance.
					This could be one of the following values: PROVISIONING, STAGING, RUNNING, STOPPING, SUSPENDING, SUSPENDED, REPAIRING, and TERMINATED.
					For more information about the status of the instance, see [Instance life cycle](https://cloud.google.com/compute/docs/instances/instance-life-cycle).</rdfs:comment>
    <rdfs:domain rdf:resource="http://example.org/onto/class/google_compute_instance_from_template"/>
    <rdfs:range rdf:resource="http://www.w3.org/2001/XMLSchema#string"/>
  </owl:DatatypeProperty>
  <owl:DatatypeProperty rdf:about="http://example.org/onto/prop/google_compute_instance_from_template_deletion_protection">
    <rdfs:label>deletion_protection</rdfs:label>
    <rdfs:comment>Whether deletion protection is enabled on this instance.</rdfs:comment>
    <rdfs:domain rdf:resource="http://example.org/onto/class/google_compute_instance_from_template"/>
    <rdfs:range rdf:resource="http://www.w3.org/2001/XMLSchema#string"/>
  </owl:DatatypeProperty>
  <owl:DatatypeProperty rdf:about="http://example.org/onto/prop/google_compute_instance_from_template_description">
    <rdfs:label>description</rdfs:label>
    <rdfs:comment>A brief description of the resource.</rdfs:comment>
    <rdfs:domain rdf:resource="http://example.org/onto/class/google_compute_instance_from_template"/>
    <rdfs:range rdf:resource="http://www.w3.org/2001/XMLSchema#string"/>
  </owl:DatatypeProperty>
  <owl:DatatypeProperty rdf:about="http://example.org/onto/prop/google_compute_instance_from_template_desired_status">
    <rdfs:label>desired_status</rdfs:label>
    <rdfs:comment>Desired status of the instance. Either "RUNNING", "SUSPENDED" or "TERMINATED".</rdfs:comment>
    <rdfs:domain rdf:resource="http://example.org/onto/class/google_compute_instance_from_template"/>
    <rdfs:range rdf:resource="http://www.w3.org/2001/XMLSchema#string"/>
  </owl:DatatypeProperty>
  <owl:DatatypeProperty rdf:about="http://example.org/onto/prop/google_compute_instance_from_template_effective_labels">
    <rdfs:label>effective_labels</rdfs:label>
    <rdfs:comment>All of labels (key/value pairs) present on the resource in GCP, including the labels configured through Terraform, other clients and services.</rdfs:comment>
    <rdfs:domain rdf:resource="http://example.org/onto/class/google_compute_instance_from_template"/>
    <rdfs:range rdf:resource="http://www.w3.org/2001/XMLSchema#string"/>
  </owl:DatatypeProperty>
  <owl:DatatypeProperty rdf:about="http://example.org/onto/prop/google_compute_instance_from_template_enable_display">
    <rdfs:label>enable_display</rdfs:label>
    <rdfs:comment>Whether the instance has virtual displays enabled.</rdfs:comment>
    <rdfs:domain rdf:resource="http://example.org/onto/class/google_compute_instance_from_template"/>
    <rdfs:range rdf:resource="http://www.w3.org/2001/XMLSchema#string"/>
  </owl:DatatypeProperty>
  <owl:DatatypeProperty rdf:about="http://example.org/onto/prop/google_compute_instance_from_template_hostname">
    <rdfs:label>hostname</rdfs:label>
    <rdfs:comment>A custom hostname for the instance. Must be a fully qualified DNS name and RFC-1035-valid. Valid format is a series of labels 1-63 characters long matching the regular expression [a-z]([-a-z0-9]*[a-z0-9]), concatenated with periods. The entire hostname must not exceed 253 characters. Changing this forces a new resource to be created.</rdfs:comment>
    <rdfs:domain rdf:resource="http://example.org/onto/class/google_compute_instance_from_template"/>
    <rdfs:range rdf:resource="http://www.w3.org/2001/XMLSchema#string"/>
  </owl:DatatypeProperty>
  <owl:DatatypeProperty rdf:about="http://example.org/onto/prop/google_compute_instance_from_template_id">
    <rdfs:label>id</rdfs:label>
    <rdfs:domain rdf:resource="http://example.org/onto/class/google_compute_instance_from_template"/>
    <rdfs:range rdf:resource="http://www.w3.org/2001/XMLSchema#string"/>
  </owl:DatatypeProperty>
  <owl:DatatypeProperty rdf:about="http://example.org/onto/prop/google_compute_instance_from_template_instance_id">
    <rdfs:label>instance_id</rdfs:label>
    <rdfs:comment>The server-assigned unique identifier of this instance.</rdfs:comment>
    <rdfs:domain rdf:resource="http://example.org/onto/class/google_compute_instance_from_template"/>
    <rdfs:range rdf:resource="http://www.w3.org/2001/XMLSchema#string"/>
  </owl:DatatypeProperty>
  <owl:DatatypeProperty rdf:about="http://example.org/onto/prop/google_compute_instance_from_template_key_revocation_action_type">
    <rdfs:label>key_revocation_action_type</rdfs:label>
    <rdfs:comment>Action to be taken when a customer's encryption key is revoked. Supports "STOP" and "NONE", with "NONE" being the default.</rdfs:comment>
    <rdfs:domain rdf:resource="http://example.org/onto/class/google_compute_instance_from_template"/>
    <rdfs:range rdf:resource="http://www.w3.org/2001/XMLSchema#string"/>
  </owl:DatatypeProperty>
  <owl:DatatypeProperty rdf:about="http://example.org/onto/prop/google_compute_instance_from_template_label_fingerprint">
    <rdfs:label>label_fingerprint</rdfs:label>
    <rdfs:comment>The unique fingerprint of the labels.</rdfs:comment>
    <rdfs:domain rdf:resource="http://example.org/onto/class/google_compute_instance_from_template"/>
    <rdfs:range rdf:resource="http://www.w3.org/2001/XMLSchema#string"/>
  </owl:DatatypeProperty>
  <owl:DatatypeProperty rdf:about="http://example.org/onto/prop/google_compute_instance_from_template_labels">
    <rdfs:label>labels</rdfs:label>
    <rdfs:comment>A set of key/value label pairs assigned to the instance.

				**Note**: This field is non-authoritative, and will only manage the labels present in your configuration.
				Please refer to the field 'effective_labels' for all of the labels present on the resource.</rdfs:comment>
    <rdfs:domain rdf:resource="http://example.org/onto/class/google_compute_instance_from_template"/>
    <rdfs:range rdf:resource="http://www.w3.org/2001/XMLSchema#string"/>
  </owl:DatatypeProperty>
  <owl:DatatypeProperty rdf:about="http://example.org/onto/prop/google_compute_instance_from_template_machine_type">
    <rdfs:label>machine_type</rdfs:label>
    <rdfs:comment>The machine type to create.</rdfs:comment>
    <rdfs:domain rdf:resource="http://example.org/onto/class/google_compute_instance_from_template"/>
    <rdfs:range rdf:resource="http://www.w3.org/2001/XMLSchema#string"/>
  </owl:DatatypeProperty>
  <owl:DatatypeProperty rdf:about="http://example.org/onto/prop/google_compute_instance_from_template_metadata">
    <rdfs:label>metadata</rdfs:label>
    <rdfs:comment>Metadata key/value pairs made available within the instance.</rdfs:comment>
    <rdfs:domain rdf:resource="http://example.org/onto/class/google_compute_instance_from_template"/>
    <rdfs:range rdf:resource="http://www.w3.org/2001/XMLSchema#string"/>
  </owl:DatatypeProperty>
  <owl:DatatypeProperty rdf:about="http://example.org/onto/prop/google_compute_instance_from_template_metadata_fingerprint">
    <rdfs:label>metadata_fingerprint</rdfs:label>
    <rdfs:comment>The unique fingerprint of the metadata.</rdfs:comment>
    <rdfs:domain rdf:resource="http://example.org/onto/class/google_compute_instance_from_template"/>
    <rdfs:range rdf:resource="http://www.w3.org/2001/XMLSchema#string"/>
  </owl:DatatypeProperty>
  <owl:DatatypeProperty rdf:about="http://example.org/onto/prop/google_compute_instance_from_template_metadata_startup_script">
    <rdfs:label>metadata_startup_script</rdfs:label>
    <rdfs:comment>Metadata startup scripts made available within the instance.</rdfs:comment>
    <rdfs:domain rdf:resource="http://example.org/onto/class/google_compute_instance_from_template"/>
    <rdfs:range rdf:resource="http://www.w3.org/2001/XMLSchema#string"/>
  </owl:DatatypeProperty>
  <owl:DatatypeProperty rdf:about="http://example.org/onto/prop/google_compute_instance_from_template_min_cpu_platform">
    <rdfs:label>min_cpu_platform</rdfs:label>
    <rdfs:comment>The minimum CPU platform specified for the VM instance.</rdfs:comment>
    <rdfs:domain rdf:resource="http://example.org/onto/class/google_compute_instance_from_template"/>
    <rdfs:range rdf:resource="http://www.w3.org/2001/XMLSchema#string"/>
  </owl:DatatypeProperty>
  <owl:DatatypeProperty rdf:about="http://example.org/onto/prop/google_compute_instance_from_template_name">
    <rdfs:label>name</rdfs:label>
    <rdfs:comment>The name of the instance. One of name or self_link must be provided.</rdfs:comment>
    <rdfs:domain rdf:resource="http://example.org/onto/class/google_compute_instance_from_template"/>
    <rdfs:range rdf:resource="http://www.w3.org/2001/XMLSchema#string"/>
  </owl:DatatypeProperty>
  <owl:DatatypeProperty rdf:about="http://example.org/onto/prop/google_compute_instance_from_template_project">
    <rdfs:label>project</rdfs:label>
    <rdfs:comment>The ID of the project in which the resource belongs. If self_link is provided, this value is ignored. If neither self_link nor project are provided, the provider project is used.</rdfs:comment>
    <rdfs:domain rdf:resource="http://example.org/onto/class/google_compute_instance_from_template"/>
    <rdfs:range rdf:resource="http://www.w3.org/2001/XMLSchema#string"/>
  </owl:DatatypeProperty>
  <owl:DatatypeProperty rdf:about="http://example.org/onto/prop/google_compute_instance_from_template_resource_policies">
    <rdfs:label>resource_policies</rdfs:label>
    <rdfs:comment>A list of self_links of resource policies to attach to the instance. Currently a max of 1 resource policy is supported.</rdfs:comment>
    <rdfs:domain rdf:resource="http://example.org/onto/class/google_compute_instance_from_template"/>
    <rdfs:range rdf:resource="http://www.w3.org/2001/XMLSchema#string"/>
  </owl:DatatypeProperty>
  <owl:DatatypeProperty rdf:about="http://example.org/onto/prop/google_compute_instance_from_template_self_link">
    <rdfs:label>self_link</rdfs:label>
    <rdfs:comment>The URI of the created resource.</rdfs:comment>
    <rdfs:domain rdf:resource="http://example.org/onto/class/google_compute_instance_from_template"/>
    <rdfs:range rdf:resource="http://www.w3.org/2001/XMLSchema#string"/>
  </owl:DatatypeProperty>
  <owl:DatatypeProperty rdf:about="http://example.org/onto/prop/google_compute_instance_from_template_source_instance_template">
    <rdfs:label>source_instance_template</rdfs:label>
    <rdfs:comment>Name or self link of an instance template to create the instance based on.</rdfs:comment>
    <rdfs:domain rdf:resource="http://example.org/onto/class/google_compute_instance_from_template"/>
    <rdfs:range rdf:resource="http://www.w3.org/2001/XMLSchema#string"/>
  </owl:DatatypeProperty>
  <owl:DatatypeProperty rdf:about="http://example.org/onto/prop/google_compute_instance_from_template_tags">
    <rdfs:label>tags</rdfs:label>
    <rdfs:comment>The list of tags attached to the instance.</rdfs:comment>
    <rdfs:domain rdf:resource="http://example.org/onto/class/google_compute_instance_from_template"/>
    <rdfs:range rdf:resource="http://www.w3.org/2001/XMLSchema#string"/>
  </owl:DatatypeProperty>
  <owl:DatatypeProperty rdf:about="http://example.org/onto/prop/google_compute_instance_from_template_tags_fingerprint">
    <rdfs:label>tags_fingerprint</rdfs:label>
    <rdfs:comment>The unique fingerprint of the tags.</rdfs:comment>
    <rdfs:domain rdf:resource="http://example.org/onto/class/google_compute_instance_from_template"/>
    <rdfs:range rdf:resource="http://www.w3.org/2001/XMLSchema#string"/>
  </owl:DatatypeProperty>
  <owl:DatatypeProperty rdf:about="http://example.org/onto/prop/google_compute_instance_from_template_terraform_labels">
    <rdfs:label>terraform_labels</rdfs:label>
    <rdfs:comment>The combination of labels configured directly on the resource and default labels configured on the provider.</rdfs:comment>
    <rdfs:domain rdf:resource="http://example.org/onto/class/google_compute_instance_from_template"/>
    <rdfs:range rdf:resource="http://www.w3.org/2001/XMLSchema#string"/>
  </owl:DatatypeProperty>
  <owl:DatatypeProperty rdf:about="http://example.org/onto/prop/google_compute_instance_from_template_zone">
    <rdfs:label>zone</rdfs:label>
    <rdfs:comment>The zone of the instance. If self_link is provided, this value is ignored. If neither self_link nor zone are provided, the provider zone is used.</rdfs:comment>
    <rdfs:domain rdf:resource="http://example.org/onto/class/google_compute_instance_from_template"/>
    <rdfs:range rdf:resource="http://www.w3.org/2001/XMLSchema#string"/>
  </owl:DatatypeProperty>
  <owl:DatatypeProperty rdf:about="http://example.org/onto/prop/google_compute_instance_from_template_enable_nested_virtualization">
    <rdfs:label>enable_nested_virtualization</rdfs:label>
    <rdfs:comment>Whether to enable nested virtualization or not.</rdfs:comment>
    <rdfs:domain rdf:resource="http://example.org/onto/class/google_compute_instance_from_template"/>
    <rdfs:range rdf:resource="http://www.w3.org/2001/XMLSchema#string"/>
  </owl:DatatypeProperty>
  <owl:DatatypeProperty rdf:about="http://example.org/onto/prop/google_compute_instance_from_template_enable_uefi_networking">
    <rdfs:label>enable_uefi_networking</rdfs:label>
    <rdfs:comment>Whether to enable UEFI networking for the instance.</rdfs:comment>
    <rdfs:domain rdf:resource="http://example.org/onto/class/google_compute_instance_from_template"/>
    <rdfs:range rdf:resource="http://www.w3.org/2001/XMLSchema#string"/>
  </owl:DatatypeProperty>
  <owl:DatatypeProperty rdf:about="http://example.org/onto/prop/google_compute_instance_from_template_performance_monitoring_unit">
    <rdfs:label>performance_monitoring_unit</rdfs:label>
    <rdfs:comment>The PMU is a hardware component within the CPU core that monitors how the processor runs code. Valid values for the level of PMU are "STANDARD", "ENHANCED", and "ARCHITECTURAL".</rdfs:comment>
    <rdfs:domain rdf:resource="http://example.org/onto/class/google_compute_instance_from_template"/>
    <rdfs:range rdf:resource="http://www.w3.org/2001/XMLSchema#string"/>
  </owl:DatatypeProperty>
  <owl:DatatypeProperty rdf:about="http://example.org/onto/prop/google_compute_instance_from_template_threads_per_core">
    <rdfs:label>threads_per_core</rdfs:label>
    <rdfs:comment>The number of threads per physical core. To disable simultaneous multithreading (SMT) set this to 1. If unset, the maximum number of threads supported per core by the underlying processor is assumed.</rdfs:comment>
    <rdfs:domain rdf:resource="http://example.org/onto/class/google_compute_instance_from_template"/>
    <rdfs:range rdf:resource="http://www.w3.org/2001/XMLSchema#string"/>
  </owl:DatatypeProperty>
  <owl:DatatypeProperty rdf:about="http://example.org/onto/prop/google_compute_instance_from_template_turbo_mode">
    <rdfs:label>turbo_mode</rdfs:label>
    <rdfs:comment>Turbo frequency mode to use for the instance. Currently supported modes is "ALL_CORE_MAX".</rdfs:comment>
    <rdfs:domain rdf:resource="http://example.org/onto/class/google_compute_instance_from_template"/>
    <rdfs:range rdf:resource="http://www.w3.org/2001/XMLSchema#string"/>
  </owl:DatatypeProperty>
  <owl:DatatypeProperty rdf:about="http://example.org/onto/prop/google_compute_instance_from_template_visible_core_count">
    <rdfs:label>visible_core_count</rdfs:label>
    <rdfs:comment>The number of physical cores to expose to an instance. Multiply by the number of threads per core to compute the total number of virtual CPUs to expose to the instance. If unset, the number of cores is inferred from the instance\'s nominal CPU count and the underlying platform\'s SMT width.</rdfs:comment>
    <rdfs:domain rdf:resource="http://example.org/onto/class/google_compute_instance_from_template"/>
    <rdfs:range rdf:resource="http://www.w3.org/2001/XMLSchema#string"/>
  </owl:DatatypeProperty>
  <owl:DatatypeProperty rdf:about="http://example.org/onto/prop/google_compute_instance_from_template_device_name">
    <rdfs:label>device_name</rdfs:label>
    <rdfs:comment>Name with which the attached disk is accessible under /dev/disk/by-id/</rdfs:comment>
    <rdfs:domain rdf:resource="http://example.org/onto/class/google_compute_instance_from_template"/>
    <rdfs:range rdf:resource="http://www.w3.org/2001/XMLSchema#string"/>
  </owl:DatatypeProperty>
  <owl:DatatypeProperty rdf:about="http://example.org/onto/prop/google_compute_instance_from_template_disk_encryption_key_raw">
    <rdfs:label>disk_encryption_key_raw</rdfs:label>
    <rdfs:comment>A 256-bit customer-supplied encryption key, encoded in RFC 4648 base64 to encrypt this disk. Only one of kms_key_self_link, disk_encryption_key_rsa and disk_encryption_key_raw may be set.</rdfs:comment>
    <rdfs:domain rdf:resource="http://example.org/onto/class/google_compute_instance_from_template"/>
    <rdfs:range rdf:resource="http://www.w3.org/2001/XMLSchema#string"/>
  </owl:DatatypeProperty>
  <owl:DatatypeProperty rdf:about="http://example.org/onto/prop/google_compute_instance_from_template_disk_encryption_key_rsa">
    <rdfs:label>disk_encryption_key_rsa</rdfs:label>
    <rdfs:comment>Specifies an RFC 4648 base64 encoded, RSA-wrapped 2048-bit customer-supplied encryption key to either encrypt or decrypt this resource. Only one of kms_key_self_link, disk_encryption_key_rsa and disk_encryption_key_raw may be set.</rdfs:comment>
    <rdfs:domain rdf:resource="http://example.org/onto/class/google_compute_instance_from_template"/>
    <rdfs:range rdf:resource="http://www.w3.org/2001/XMLSchema#string"/>
  </owl:DatatypeProperty>
  <owl:DatatypeProperty rdf:about="http://example.org/onto/prop/google_compute_instance_from_template_disk_encryption_key_sha256">
    <rdfs:label>disk_encryption_key_sha256</rdfs:label>
    <rdfs:comment>The RFC 4648 base64 encoded SHA-256 hash of the customer-supplied encryption key that protects this resource.</rdfs:comment>
    <rdfs:domain rdf:resource="http://example.org/onto/class/google_compute_instance_from_template"/>
    <rdfs:range rdf:resource="http://www.w3.org/2001/XMLSchema#string"/>
  </owl:DatatypeProperty>
  <owl:DatatypeProperty rdf:about="http://example.org/onto/prop/google_compute_instance_from_template_disk_encryption_service_account">
    <rdfs:label>disk_encryption_service_account</rdfs:label>
    <rdfs:comment>The service account being used for the encryption request for the given KMS key. If absent, the Compute Engine default service account is used</rdfs:comment>
    <rdfs:domain rdf:resource="http://example.org/onto/class/google_compute_instance_from_template"/>
    <rdfs:range rdf:resource="http://www.w3.org/2001/XMLSchema#string"/>
  </owl:DatatypeProperty>
  <owl:DatatypeProperty rdf:about="http://example.org/onto/prop/google_compute_instance_from_template_force_attach">
    <rdfs:label>force_attach</rdfs:label>
    <rdfs:comment>Whether to force attach the regional disk even if it's currently attached to another instance. If you try to force attach a zonal disk to an instance, you will receive an error. Setting this parameter cause VM recreation.</rdfs:comment>
    <rdfs:domain rdf:resource="http://example.org/onto/class/google_compute_instance_from_template"/>
    <rdfs:range rdf:resource="http://www.w3.org/2001/XMLSchema#string"/>
  </owl:DatatypeProperty>
  <owl:DatatypeProperty rdf:about="http://example.org/onto/prop/google_compute_instance_from_template_kms_key_self_link">
    <rdfs:label>kms_key_self_link</rdfs:label>
    <rdfs:comment>The self_link of the encryption key that is stored in Google Cloud KMS to encrypt this disk. Only one of kms_key_self_link, disk_encryption_key_rsa and disk_encryption_key_raw may be set.</rdfs:comment>
    <rdfs:domain rdf:resource="http://example.org/onto/class/google_compute_instance_from_template"/>
    <rdfs:range rdf:resource="http://www.w3.org/2001/XMLSchema#string"/>
  </owl:DatatypeProperty>
  <owl:DatatypeProperty rdf:about="http://example.org/onto/prop/google_compute_instance_from_template_mode">
    <rdfs:label>mode</rdfs:label>
    <rdfs:comment>Read/write mode for the disk. One of "READ_ONLY" or "READ_WRITE".</rdfs:comment>
    <rdfs:domain rdf:resource="http://example.org/onto/class/google_compute_instance_from_template"/>
    <rdfs:range rdf:resource="http://www.w3.org/2001/XMLSchema#string"/>
  </owl:DatatypeProperty>
  <owl:DatatypeProperty rdf:about="http://example.org/onto/prop/google_compute_instance_from_template_source">
    <rdfs:label>source</rdfs:label>
    <rdfs:comment>The name or self_link of the disk attached to this instance.</rdfs:comment>
    <rdfs:domain rdf:resource="http://example.org/onto/class/google_compute_instance_from_template"/>
    <rdfs:range rdf:resource="http://www.w3.org/2001/XMLSchema#string"/>
  </owl:DatatypeProperty>
  <owl:DatatypeProperty rdf:about="http://example.org/onto/prop/google_compute_instance_from_template_auto_delete">
    <rdfs:label>auto_delete</rdfs:label>
    <rdfs:comment>Whether the disk will be auto-deleted when the instance is deleted.</rdfs:comment>
    <rdfs:domain rdf:resource="http://example.org/onto/class/google_compute_instance_from_template"/>
    <rdfs:range rdf:resource="http://www.w3.org/2001/XMLSchema#string"/>
  </owl:DatatypeProperty>
  <owl:DatatypeProperty rdf:about="http://example.org/onto/prop/google_compute_instance_from_template_device_name">
    <rdfs:label>device_name</rdfs:label>
    <rdfs:comment>Name with which attached disk will be accessible under /dev/disk/by-id/</rdfs:comment>
    <rdfs:domain rdf:resource="http://example.org/onto/class/google_compute_instance_from_template"/>
    <rdfs:range rdf:resource="http://www.w3.org/2001/XMLSchema#string"/>
  </owl:DatatypeProperty>
  <owl:DatatypeProperty rdf:about="http://example.org/onto/prop/google_compute_instance_from_template_disk_encryption_key_raw">
    <rdfs:label>disk_encryption_key_raw</rdfs:label>
    <rdfs:comment>A 256-bit customer-supplied encryption key, encoded in RFC 4648 base64 to encrypt this disk. Only one of kms_key_self_link, disk_encryption_key_raw and disk_encryption_key_rsa may be set.</rdfs:comment>
    <rdfs:domain rdf:resource="http://example.org/onto/class/google_compute_instance_from_template"/>
    <rdfs:range rdf:resource="http://www.w3.org/2001/XMLSchema#string"/>
  </owl:DatatypeProperty>
  <owl:DatatypeProperty rdf:about="http://example.org/onto/prop/google_compute_instance_from_template_disk_encryption_key_rsa">
    <rdfs:label>disk_encryption_key_rsa</rdfs:label>
    <rdfs:comment>Specifies an RFC 4648 base64 encoded, RSA-wrapped 2048-bit customer-supplied encryption key to either encrypt or decrypt this resource. Only one of kms_key_self_link, disk_encryption_key_raw and disk_encryption_key_rsa may be set.</rdfs:comment>
    <rdfs:domain rdf:resource="http://example.org/onto/class/google_compute_instance_from_template"/>
    <rdfs:range rdf:resource="http://www.w3.org/2001/XMLSchema#string"/>
  </owl:DatatypeProperty>
  <owl:DatatypeProperty rdf:about="http://example.org/onto/prop/google_compute_instance_from_template_disk_encryption_key_sha256">
    <rdfs:label>disk_encryption_key_sha256</rdfs:label>
    <rdfs:comment>The RFC 4648 base64 encoded SHA-256 hash of the customer-supplied encryption key that protects this resource.</rdfs:comment>
    <rdfs:domain rdf:resource="http://example.org/onto/class/google_compute_instance_from_template"/>
    <rdfs:range rdf:resource="http://www.w3.org/2001/XMLSchema#string"/>
  </owl:DatatypeProperty>
  <owl:DatatypeProperty rdf:about="http://example.org/onto/prop/google_compute_instance_from_template_disk_encryption_service_account">
    <rdfs:label>disk_encryption_service_account</rdfs:label>
    <rdfs:comment>The service account being used for the encryption request for the given KMS key. If absent, the Compute Engine default service account is used</rdfs:comment>
    <rdfs:domain rdf:resource="http://example.org/onto/class/google_compute_instance_from_template"/>
    <rdfs:range rdf:resource="http://www.w3.org/2001/XMLSchema#string"/>
  </owl:DatatypeProperty>
  <owl:DatatypeProperty rdf:about="http://example.org/onto/prop/google_compute_instance_from_template_force_attach">
    <rdfs:label>force_attach</rdfs:label>
    <rdfs:comment>Whether to force attach the regional disk even if it's currently attached to another instance. If you try to force attach a zonal disk to an instance, you will receive an error. Setting this parameter cause VM recreation.</rdfs:comment>
    <rdfs:domain rdf:resource="http://example.org/onto/class/google_compute_instance_from_template"/>
    <rdfs:range rdf:resource="http://www.w3.org/2001/XMLSchema#string"/>
  </owl:DatatypeProperty>
  <owl:DatatypeProperty rdf:about="http://example.org/onto/prop/google_compute_instance_from_template_guest_os_features">
    <rdfs:label>guest_os_features</rdfs:label>
    <rdfs:comment>A list of features to enable on the guest operating system. Applicable only for bootable images.</rdfs:comment>
    <rdfs:domain rdf:resource="http://example.org/onto/class/google_compute_instance_from_template"/>
    <rdfs:range rdf:resource="http://www.w3.org/2001/XMLSchema#string"/>
  </owl:DatatypeProperty>
  <owl:DatatypeProperty rdf:about="http://example.org/onto/prop/google_compute_instance_from_template_interface">
    <rdfs:label>interface</rdfs:label>
    <rdfs:comment>The disk interface used for attaching this disk. One of SCSI or NVME. (This field is shared with attached_disk and only used for specific cases, please don't specify this field without advice from Google.)</rdfs:comment>
    <rdfs:domain rdf:resource="http://example.org/onto/class/google_compute_instance_from_template"/>
    <rdfs:range rdf:resource="http://www.w3.org/2001/XMLSchema#string"/>
  </owl:DatatypeProperty>
  <owl:DatatypeProperty rdf:about="http://example.org/onto/prop/google_compute_instance_from_template_kms_key_self_link">
    <rdfs:label>kms_key_self_link</rdfs:label>
    <rdfs:comment>The self_link of the encryption key that is stored in Google Cloud KMS to encrypt this disk. Only one of kms_key_self_link, disk_encryption_key_raw and disk_encryption_key_rsa may be set.</rdfs:comment>
    <rdfs:domain rdf:resource="http://example.org/onto/class/google_compute_instance_from_template"/>
    <rdfs:range rdf:resource="http://www.w3.org/2001/XMLSchema#string"/>
  </owl:DatatypeProperty>
  <owl:DatatypeProperty rdf:about="http://example.org/onto/prop/google_compute_instance_from_template_mode">
    <rdfs:label>mode</rdfs:label>
    <rdfs:comment>Read/write mode for the disk. One of "READ_ONLY" or "READ_WRITE".</rdfs:comment>
    <rdfs:domain rdf:resource="http://example.org/onto/class/google_compute_instance_from_template"/>
    <rdfs:range rdf:resource="http://www.w3.org/2001/XMLSchema#string"/>
  </owl:DatatypeProperty>
  <owl:DatatypeProperty rdf:about="http://example.org/onto/prop/google_compute_instance_from_template_source">
    <rdfs:label>source</rdfs:label>
    <rdfs:comment>The name or self_link of the disk attached to this instance.</rdfs:comment>
    <rdfs:domain rdf:resource="http://example.org/onto/class/google_compute_instance_from_template"/>
    <rdfs:range rdf:resource="http://www.w3.org/2001/XMLSchema#string"/>
  </owl:DatatypeProperty>
  <owl:DatatypeProperty rdf:about="http://example.org/onto/prop/google_compute_instance_from_template_architecture">
    <rdfs:label>architecture</rdfs:label>
    <rdfs:comment>The architecture of the disk. One of "X86_64" or "ARM64".</rdfs:comment>
    <rdfs:domain rdf:resource="http://example.org/onto/class/google_compute_instance_from_template"/>
    <rdfs:range rdf:resource="http://www.w3.org/2001/XMLSchema#string"/>
  </owl:DatatypeProperty>
  <owl:DatatypeProperty rdf:about="http://example.org/onto/prop/google_compute_instance_from_template_enable_confidential_compute">
    <rdfs:label>enable_confidential_compute</rdfs:label>
    <rdfs:comment>A flag to enable confidential compute mode on boot disk</rdfs:comment>
    <rdfs:domain rdf:resource="http://example.org/onto/class/google_compute_instance_from_template"/>
    <rdfs:range rdf:resource="http://www.w3.org/2001/XMLSchema#string"/>
  </owl:DatatypeProperty>
  <owl:DatatypeProperty rdf:about="http://example.org/onto/prop/google_compute_instance_from_template_image">
    <rdfs:label>image</rdfs:label>
    <rdfs:comment>The image from which this disk was initialised.</rdfs:comment>
    <rdfs:domain rdf:resource="http://example.org/onto/class/google_compute_instance_from_template"/>
    <rdfs:range rdf:resource="http://www.w3.org/2001/XMLSchema#string"/>
  </owl:DatatypeProperty>
  <owl:DatatypeProperty rdf:about="http://example.org/onto/prop/google_compute_instance_from_template_labels">
    <rdfs:label>labels</rdfs:label>
    <rdfs:comment>A set of key/value label pairs assigned to the disk.</rdfs:comment>
    <rdfs:domain rdf:resource="http://example.org/onto/class/google_compute_instance_from_template"/>
    <rdfs:range rdf:resource="http://www.w3.org/2001/XMLSchema#string"/>
  </owl:DatatypeProperty>
  <owl:DatatypeProperty rdf:about="http://example.org/onto/prop/google_compute_instance_from_template_provisioned_iops">
    <rdfs:label>provisioned_iops</rdfs:label>
    <rdfs:comment>Indicates how many IOPS to provision for the disk. This sets the number of I/O operations per second that the disk can handle.</rdfs:comment>
    <rdfs:domain rdf:resource="http://example.org/onto/class/google_compute_instance_from_template"/>
    <rdfs:range rdf:resource="http://www.w3.org/2001/XMLSchema#string"/>
  </owl:DatatypeProperty>
  <owl:DatatypeProperty rdf:about="http://example.org/onto/prop/google_compute_instance_from_template_provisioned_throughput">
    <rdfs:label>provisioned_throughput</rdfs:label>
    <rdfs:comment>Indicates how much throughput to provision for the disk. This sets the number of throughput mb per second that the disk can handle.</rdfs:comment>
    <rdfs:domain rdf:resource="http://example.org/onto/class/google_compute_instance_from_template"/>
    <rdfs:range rdf:resource="http://www.w3.org/2001/XMLSchema#string"/>
  </owl:DatatypeProperty>
  <owl:DatatypeProperty rdf:about="http://example.org/onto/prop/google_compute_instance_from_template_resource_manager_tags">
    <rdfs:label>resource_manager_tags</rdfs:label>
    <rdfs:comment>A map of resource manager tags. Resource manager tag keys and values have the same definition as resource manager tags. Keys must be in the format tagKeys/{tag_key_id}, and values are in the format tagValues/456. The field is ignored (both PUT & PATCH) when empty.</rdfs:comment>
    <rdfs:domain rdf:resource="http://example.org/onto/class/google_compute_instance_from_template"/>
    <rdfs:range rdf:resource="http://www.w3.org/2001/XMLSchema#string"/>
  </owl:DatatypeProperty>
  <owl:DatatypeProperty rdf:about="http://example.org/onto/prop/google_compute_instance_from_template_resource_policies">
    <rdfs:label>resource_policies</rdfs:label>
    <rdfs:comment>A list of self_links of resource policies to attach to the instance's boot disk. Modifying this list will cause the instance to recreate. Currently a max of 1 resource policy is supported.</rdfs:comment>
    <rdfs:domain rdf:resource="http://example.org/onto/class/google_compute_instance_from_template"/>
    <rdfs:range rdf:resource="http://www.w3.org/2001/XMLSchema#string"/>
  </owl:DatatypeProperty>
  <owl:DatatypeProperty rdf:about="http://example.org/onto/prop/google_compute_instance_from_template_size">
    <rdfs:label>size</rdfs:label>
    <rdfs:comment>The size of the image in gigabytes.</rdfs:comment>
    <rdfs:domain rdf:resource="http://example.org/onto/class/google_compute_instance_from_template"/>
    <rdfs:range rdf:resource="http://www.w3.org/2001/XMLSchema#string"/>
  </owl:DatatypeProperty>
  <owl:DatatypeProperty rdf:about="http://example.org/onto/prop/google_compute_instance_from_template_snapshot">
    <rdfs:label>snapshot</rdfs:label>
    <rdfs:comment>The snapshot from which this disk was initialised.</rdfs:comment>
    <rdfs:domain rdf:resource="http://example.org/onto/class/google_compute_instance_from_template"/>
    <rdfs:range rdf:resource="http://www.w3.org/2001/XMLSchema#string"/>
  </owl:DatatypeProperty>
  <owl:DatatypeProperty rdf:about="http://example.org/onto/prop/google_compute_instance_from_template_storage_pool">
    <rdfs:label>storage_pool</rdfs:label>
    <rdfs:comment>The URL of the storage pool in which the new disk is created</rdfs:comment>
    <rdfs:domain rdf:resource="http://example.org/onto/class/google_compute_instance_from_template"/>
    <rdfs:range rdf:resource="http://www.w3.org/2001/XMLSchema#string"/>
  </owl:DatatypeProperty>
  <owl:DatatypeProperty rdf:about="http://example.org/onto/prop/google_compute_instance_from_template_type">
    <rdfs:label>type</rdfs:label>
    <rdfs:comment>The Google Compute Engine disk type. Such as pd-standard, pd-ssd or pd-balanced.</rdfs:comment>
    <rdfs:domain rdf:resource="http://example.org/onto/class/google_compute_instance_from_template"/>
    <rdfs:range rdf:resource="http://www.w3.org/2001/XMLSchema#string"/>
  </owl:DatatypeProperty>
  <owl:DatatypeProperty rdf:about="http://example.org/onto/prop/google_compute_instance_from_template_kms_key_self_link">
    <rdfs:label>kms_key_self_link</rdfs:label>
    <rdfs:comment>The self link of the encryption key that is stored in Google Cloud KMS. Only one of kms_key_self_link, rsa_encrypted_key and raw_key may be set.</rdfs:comment>
    <rdfs:domain rdf:resource="http://example.org/onto/class/google_compute_instance_from_template"/>
    <rdfs:range rdf:resource="http://www.w3.org/2001/XMLSchema#string"/>
  </owl:DatatypeProperty>
  <owl:DatatypeProperty rdf:about="http://example.org/onto/prop/google_compute_instance_from_template_kms_key_service_account">
    <rdfs:label>kms_key_service_account</rdfs:label>
    <rdfs:comment>The service account being used for the encryption request for the given KMS key. If absent, the Compute Engine default service account is used.</rdfs:comment>
    <rdfs:domain rdf:resource="http://example.org/onto/class/google_compute_instance_from_template"/>
    <rdfs:range rdf:resource="http://www.w3.org/2001/XMLSchema#string"/>
  </owl:DatatypeProperty>
  <owl:DatatypeProperty rdf:about="http://example.org/onto/prop/google_compute_instance_from_template_raw_key">
    <rdfs:label>raw_key</rdfs:label>
    <rdfs:comment>Specifies a 256-bit customer-supplied encryption key, encoded in RFC 4648 base64 to either encrypt or decrypt this resource. Only one of kms_key_self_link, rsa_encrypted_key and raw_key may be set.</rdfs:comment>
    <rdfs:domain rdf:resource="http://example.org/onto/class/google_compute_instance_from_template"/>
    <rdfs:range rdf:resource="http://www.w3.org/2001/XMLSchema#string"/>
  </owl:DatatypeProperty>
  <owl:DatatypeProperty rdf:about="http://example.org/onto/prop/google_compute_instance_from_template_rsa_encrypted_key">
    <rdfs:label>rsa_encrypted_key</rdfs:label>
    <rdfs:comment>Specifies an RFC 4648 base64 encoded, RSA-wrapped 2048-bit customer-supplied encryption key to either encrypt or decrypt this resource. Only one of kms_key_self_link, rsa_encrypted_key and raw_key may be set.</rdfs:comment>
    <rdfs:domain rdf:resource="http://example.org/onto/class/google_compute_instance_from_template"/>
    <rdfs:range rdf:resource="http://www.w3.org/2001/XMLSchema#string"/>
  </owl:DatatypeProperty>
  <owl:DatatypeProperty rdf:about="http://example.org/onto/prop/google_compute_instance_from_template_sha256">
    <rdfs:label>sha256</rdfs:label>
    <rdfs:comment>The SHA256 hash of the encryption key used to encrypt this disk.</rdfs:comment>
    <rdfs:domain rdf:resource="http://example.org/onto/class/google_compute_instance_from_template"/>
    <rdfs:range rdf:resource="http://www.w3.org/2001/XMLSchema#string"/>
  </owl:DatatypeProperty>
  <owl:DatatypeProperty rdf:about="http://example.org/onto/prop/google_compute_instance_from_template_kms_key_self_link">
    <rdfs:label>kms_key_self_link</rdfs:label>
    <rdfs:comment>The self link of the encryption key that is stored in Google Cloud KMS. Only one of kms_key_self_link, rsa_encrypted_key and raw_key may be set.</rdfs:comment>
    <rdfs:domain rdf:resource="http://example.org/onto/class/google_compute_instance_from_template"/>
    <rdfs:range rdf:resource="http://www.w3.org/2001/XMLSchema#string"/>
  </owl:DatatypeProperty>
  <owl:DatatypeProperty rdf:about="http://example.org/onto/prop/google_compute_instance_from_template_kms_key_service_account">
    <rdfs:label>kms_key_service_account</rdfs:label>
    <rdfs:comment>The service account being used for the encryption request for the given KMS key. If absent, the Compute Engine default service account is used.</rdfs:comment>
    <rdfs:domain rdf:resource="http://example.org/onto/class/google_compute_instance_from_template"/>
    <rdfs:range rdf:resource="http://www.w3.org/2001/XMLSchema#string"/>
  </owl:DatatypeProperty>
  <owl:DatatypeProperty rdf:about="http://example.org/onto/prop/google_compute_instance_from_template_raw_key">
    <rdfs:label>raw_key</rdfs:label>
    <rdfs:comment>Specifies a 256-bit customer-supplied encryption key, encoded in RFC 4648 base64 to either encrypt or decrypt this resource. Only one of kms_key_self_link, rsa_encrypted_key and raw_key may be set.</rdfs:comment>
    <rdfs:domain rdf:resource="http://example.org/onto/class/google_compute_instance_from_template"/>
    <rdfs:range rdf:resource="http://www.w3.org/2001/XMLSchema#string"/>
  </owl:DatatypeProperty>
  <owl:DatatypeProperty rdf:about="http://example.org/onto/prop/google_compute_instance_from_template_rsa_encrypted_key">
    <rdfs:label>rsa_encrypted_key</rdfs:label>
    <rdfs:comment>Specifies an RFC 4648 base64 encoded, RSA-wrapped 2048-bit customer-supplied encryption key to either encrypt or decrypt this resource. Only one of kms_key_self_link, rsa_encrypted_key and raw_key may be set.</rdfs:comment>
    <rdfs:domain rdf:resource="http://example.org/onto/class/google_compute_instance_from_template"/>
    <rdfs:range rdf:resource="http://www.w3.org/2001/XMLSchema#string"/>
  </owl:DatatypeProperty>
  <owl:DatatypeProperty rdf:about="http://example.org/onto/prop/google_compute_instance_from_template_sha256">
    <rdfs:label>sha256</rdfs:label>
    <rdfs:comment>The SHA256 hash of the encryption key used to encrypt this disk.</rdfs:comment>
    <rdfs:domain rdf:resource="http://example.org/onto/class/google_compute_instance_from_template"/>
    <rdfs:range rdf:resource="http://www.w3.org/2001/XMLSchema#string"/>
  </owl:DatatypeProperty>
  <owl:DatatypeProperty rdf:about="http://example.org/onto/prop/google_compute_instance_from_template_confidential_instance_type">
    <rdfs:label>confidential_instance_type</rdfs:label>
    <rdfs:comment>The confidential computing technology the instance uses.
								SEV is an AMD feature. TDX is an Intel feature. One of the following
								values is required: SEV, SEV_SNP, TDX. If SEV_SNP, min_cpu_platform =
								"AMD Milan" is currently required.</rdfs:comment>
    <rdfs:domain rdf:resource="http://example.org/onto/class/google_compute_instance_from_template"/>
    <rdfs:range rdf:resource="http://www.w3.org/2001/XMLSchema#string"/>
  </owl:DatatypeProperty>
  <owl:DatatypeProperty rdf:about="http://example.org/onto/prop/google_compute_instance_from_template_enable_confidential_compute">
    <rdfs:label>enable_confidential_compute</rdfs:label>
    <rdfs:comment>Defines whether the instance should have confidential compute enabled. Field will be deprecated in a future release</rdfs:comment>
    <rdfs:domain rdf:resource="http://example.org/onto/class/google_compute_instance_from_template"/>
    <rdfs:range rdf:resource="http://www.w3.org/2001/XMLSchema#string"/>
  </owl:DatatypeProperty>
  <owl:DatatypeProperty rdf:about="http://example.org/onto/prop/google_compute_instance_from_template_count">
    <rdfs:label>count</rdfs:label>
    <rdfs:comment>The number of the guest accelerator cards exposed to this instance.</rdfs:comment>
    <rdfs:domain rdf:resource="http://example.org/onto/class/google_compute_instance_from_template"/>
    <rdfs:range rdf:resource="http://www.w3.org/2001/XMLSchema#string"/>
  </owl:DatatypeProperty>
  <owl:DatatypeProperty rdf:about="http://example.org/onto/prop/google_compute_instance_from_template_type">
    <rdfs:label>type</rdfs:label>
    <rdfs:comment>The accelerator type resource exposed to this instance. E.g. nvidia-tesla-k80.</rdfs:comment>
    <rdfs:domain rdf:resource="http://example.org/onto/class/google_compute_instance_from_template"/>
    <rdfs:range rdf:resource="http://www.w3.org/2001/XMLSchema#string"/>
  </owl:DatatypeProperty>
  <owl:DatatypeProperty rdf:about="http://example.org/onto/prop/google_compute_instance_from_template_kms_key_self_link">
    <rdfs:label>kms_key_self_link</rdfs:label>
    <rdfs:comment>The self link of the encryption key that is stored in Google Cloud KMS.</rdfs:comment>
    <rdfs:domain rdf:resource="http://example.org/onto/class/google_compute_instance_from_template"/>
    <rdfs:range rdf:resource="http://www.w3.org/2001/XMLSchema#string"/>
  </owl:DatatypeProperty>
  <owl:DatatypeProperty rdf:about="http://example.org/onto/prop/google_compute_instance_from_template_kms_key_service_account">
    <rdfs:label>kms_key_service_account</rdfs:label>
    <rdfs:comment>The service account being used for the encryption request for the given KMS key. If absent, the Compute Engine default service account is used.</rdfs:comment>
    <rdfs:domain rdf:resource="http://example.org/onto/class/google_compute_instance_from_template"/>
    <rdfs:range rdf:resource="http://www.w3.org/2001/XMLSchema#string"/>
  </owl:DatatypeProperty>
  <owl:DatatypeProperty rdf:about="http://example.org/onto/prop/google_compute_instance_from_template_sha256">
    <rdfs:label>sha256</rdfs:label>
    <rdfs:comment>The SHA256 hash of the customer's encryption key.</rdfs:comment>
    <rdfs:domain rdf:resource="http://example.org/onto/class/google_compute_instance_from_template"/>
    <rdfs:range rdf:resource="http://www.w3.org/2001/XMLSchema#string"/>
  </owl:DatatypeProperty>
  <owl:DatatypeProperty rdf:about="http://example.org/onto/prop/google_compute_instance_from_template_internal_ipv6_prefix_length">
    <rdfs:label>internal_ipv6_prefix_length</rdfs:label>
    <rdfs:comment>The prefix length of the primary internal IPv6 range.</rdfs:comment>
    <rdfs:domain rdf:resource="http://example.org/onto/class/google_compute_instance_from_template"/>
    <rdfs:range rdf:resource="http://www.w3.org/2001/XMLSchema#string"/>
  </owl:DatatypeProperty>
  <owl:DatatypeProperty rdf:about="http://example.org/onto/prop/google_compute_instance_from_template_ipv6_access_type">
    <rdfs:label>ipv6_access_type</rdfs:label>
    <rdfs:comment>One of EXTERNAL, INTERNAL to indicate whether the IP can be accessed from the Internet. This field is always inherited from its subnetwork.</rdfs:comment>
    <rdfs:domain rdf:resource="http://example.org/onto/class/google_compute_instance_from_template"/>
    <rdfs:range rdf:resource="http://www.w3.org/2001/XMLSchema#string"/>
  </owl:DatatypeProperty>
  <owl:DatatypeProperty rdf:about="http://example.org/onto/prop/google_compute_instance_from_template_ipv6_address">
    <rdfs:label>ipv6_address</rdfs:label>
    <rdfs:comment>An IPv6 internal network address for this network interface. If not specified, Google Cloud will automatically assign an internal IPv6 address from the instance's subnetwork.</rdfs:comment>
    <rdfs:domain rdf:resource="http://example.org/onto/class/google_compute_instance_from_template"/>
    <rdfs:range rdf:resource="http://www.w3.org/2001/XMLSchema#string"/>
  </owl:DatatypeProperty>
  <owl:DatatypeProperty rdf:about="http://example.org/onto/prop/google_compute_instance_from_template_name">
    <rdfs:label>name</rdfs:label>
    <rdfs:comment>The name of the interface</rdfs:comment>
    <rdfs:domain rdf:resource="http://example.org/onto/class/google_compute_instance_from_template"/>
    <rdfs:range rdf:resource="http://www.w3.org/2001/XMLSchema#string"/>
  </owl:DatatypeProperty>
  <owl:DatatypeProperty rdf:about="http://example.org/onto/prop/google_compute_instance_from_template_network">
    <rdfs:label>network</rdfs:label>
    <rdfs:comment>The name or self_link of the network attached to this interface.</rdfs:comment>
    <rdfs:domain rdf:resource="http://example.org/onto/class/google_compute_instance_from_template"/>
    <rdfs:range rdf:resource="http://www.w3.org/2001/XMLSchema#string"/>
  </owl:DatatypeProperty>
  <owl:DatatypeProperty rdf:about="http://example.org/onto/prop/google_compute_instance_from_template_network_attachment">
    <rdfs:label>network_attachment</rdfs:label>
    <rdfs:comment>The URL of the network attachment that this interface should connect to in the following format: projects/{projectNumber}/regions/{region_name}/networkAttachments/{network_attachment_name}.</rdfs:comment>
    <rdfs:domain rdf:resource="http://example.org/onto/class/google_compute_instance_from_template"/>
    <rdfs:range rdf:resource="http://www.w3.org/2001/XMLSchema#string"/>
  </owl:DatatypeProperty>
  <owl:DatatypeProperty rdf:about="http://example.org/onto/prop/google_compute_instance_from_template_network_ip">
    <rdfs:label>network_ip</rdfs:label>
    <rdfs:comment>The private IP address assigned to the instance.</rdfs:comment>
    <rdfs:domain rdf:resource="http://example.org/onto/class/google_compute_instance_from_template"/>
    <rdfs:range rdf:resource="http://www.w3.org/2001/XMLSchema#string"/>
  </owl:DatatypeProperty>
  <owl:DatatypeProperty rdf:about="http://example.org/onto/prop/google_compute_instance_from_template_nic_type">
    <rdfs:label>nic_type</rdfs:label>
    <rdfs:comment>The type of vNIC to be used on this interface. Possible values:GVNIC, VIRTIO_NET, IDPF, MRDMA, and IRDMA</rdfs:comment>
    <rdfs:domain rdf:resource="http://example.org/onto/class/google_compute_instance_from_template"/>
    <rdfs:range rdf:resource="http://www.w3.org/2001/XMLSchema#string"/>
  </owl:DatatypeProperty>
  <owl:DatatypeProperty rdf:about="http://example.org/onto/prop/google_compute_instance_from_template_queue_count">
    <rdfs:label>queue_count</rdfs:label>
    <rdfs:comment>The networking queue count that's specified by users for the network interface. Both Rx and Tx queues will be set to this number. It will be empty if not specified.</rdfs:comment>
    <rdfs:domain rdf:resource="http://example.org/onto/class/google_compute_instance_from_template"/>
    <rdfs:range rdf:resource="http://www.w3.org/2001/XMLSchema#string"/>
  </owl:DatatypeProperty>
  <owl:DatatypeProperty rdf:about="http://example.org/onto/prop/google_compute_instance_from_template_stack_type">
    <rdfs:label>stack_type</rdfs:label>
    <rdfs:comment>The stack type for this network interface to identify whether the IPv6 feature is enabled or not. If not specified, IPV4_ONLY will be used.</rdfs:comment>
    <rdfs:domain rdf:resource="http://example.org/onto/class/google_compute_instance_from_template"/>
    <rdfs:range rdf:resource="http://www.w3.org/2001/XMLSchema#string"/>
  </owl:DatatypeProperty>
  <owl:DatatypeProperty rdf:about="http://example.org/onto/prop/google_compute_instance_from_template_subnetwork">
    <rdfs:label>subnetwork</rdfs:label>
    <rdfs:comment>The name or self_link of the subnetwork attached to this interface.</rdfs:comment>
    <rdfs:domain rdf:resource="http://example.org/onto/class/google_compute_instance_from_template"/>
    <rdfs:range rdf:resource="http://www.w3.org/2001/XMLSchema#string"/>
  </owl:DatatypeProperty>
  <owl:DatatypeProperty rdf:about="http://example.org/onto/prop/google_compute_instance_from_template_subnetwork_project">
    <rdfs:label>subnetwork_project</rdfs:label>
    <rdfs:comment>The project in which the subnetwork belongs.</rdfs:comment>
    <rdfs:domain rdf:resource="http://example.org/onto/class/google_compute_instance_from_template"/>
    <rdfs:range rdf:resource="http://www.w3.org/2001/XMLSchema#string"/>
  </owl:DatatypeProperty>
  <owl:DatatypeProperty rdf:about="http://example.org/onto/prop/google_compute_instance_from_template_nat_ip">
    <rdfs:label>nat_ip</rdfs:label>
    <rdfs:comment>The IP address that is be 1:1 mapped to the instance's network ip.</rdfs:comment>
    <rdfs:domain rdf:resource="http://example.org/onto/class/google_compute_instance_from_template"/>
    <rdfs:range rdf:resource="http://www.w3.org/2001/XMLSchema#string"/>
  </owl:DatatypeProperty>
  <owl:DatatypeProperty rdf:about="http://example.org/onto/prop/google_compute_instance_from_template_network_tier">
    <rdfs:label>network_tier</rdfs:label>
    <rdfs:comment>The networking tier used for configuring this instance. One of PREMIUM or STANDARD.</rdfs:comment>
    <rdfs:domain rdf:resource="http://example.org/onto/class/google_compute_instance_from_template"/>
    <rdfs:range rdf:resource="http://www.w3.org/2001/XMLSchema#string"/>
  </owl:DatatypeProperty>
  <owl:DatatypeProperty rdf:about="http://example.org/onto/prop/google_compute_instance_from_template_public_ptr_domain_name">
    <rdfs:label>public_ptr_domain_name</rdfs:label>
    <rdfs:comment>The DNS domain name for the public PTR record.</rdfs:comment>
    <rdfs:domain rdf:resource="http://example.org/onto/class/google_compute_instance_from_template"/>
    <rdfs:range rdf:resource="http://www.w3.org/2001/XMLSchema#string"/>
  </owl:DatatypeProperty>
  <owl:DatatypeProperty rdf:about="http://example.org/onto/prop/google_compute_instance_from_template_ip_cidr_range">
    <rdfs:label>ip_cidr_range</rdfs:label>
    <rdfs:comment>The IP CIDR range represented by this alias IP range.</rdfs:comment>
    <rdfs:domain rdf:resource="http://example.org/onto/class/google_compute_instance_from_template"/>
    <rdfs:range rdf:resource="http://www.w3.org/2001/XMLSchema#string"/>
  </owl:DatatypeProperty>
  <owl:DatatypeProperty rdf:about="http://example.org/onto/prop/google_compute_instance_from_template_subnetwork_range_name">
    <rdfs:label>subnetwork_range_name</rdfs:label>
    <rdfs:comment>The subnetwork secondary range name specifying the secondary range from which to allocate the IP CIDR range for this alias IP range.</rdfs:comment>
    <rdfs:domain rdf:resource="http://example.org/onto/class/google_compute_instance_from_template"/>
    <rdfs:range rdf:resource="http://www.w3.org/2001/XMLSchema#string"/>
  </owl:DatatypeProperty>
  <owl:DatatypeProperty rdf:about="http://example.org/onto/prop/google_compute_instance_from_template_external_ipv6">
    <rdfs:label>external_ipv6</rdfs:label>
    <rdfs:comment>The first IPv6 address of the external IPv6 range associated with this instance, prefix length is stored in externalIpv6PrefixLength in ipv6AccessConfig. To use a static external IP address, it must be unused and in the same region as the instance's zone. If not specified, Google Cloud will automatically assign an external IPv6 address from the instance's subnetwork.</rdfs:comment>
    <rdfs:domain rdf:resource="http://example.org/onto/class/google_compute_instance_from_template"/>
    <rdfs:range rdf:resource="http://www.w3.org/2001/XMLSchema#string"/>
  </owl:DatatypeProperty>
  <owl:DatatypeProperty rdf:about="http://example.org/onto/prop/google_compute_instance_from_template_external_ipv6_prefix_length">
    <rdfs:label>external_ipv6_prefix_length</rdfs:label>
    <rdfs:comment>The prefix length of the external IPv6 range.</rdfs:comment>
    <rdfs:domain rdf:resource="http://example.org/onto/class/google_compute_instance_from_template"/>
    <rdfs:range rdf:resource="http://www.w3.org/2001/XMLSchema#string"/>
  </owl:DatatypeProperty>
  <owl:DatatypeProperty rdf:about="http://example.org/onto/prop/google_compute_instance_from_template_name">
    <rdfs:label>name</rdfs:label>
    <rdfs:comment>The name of this access configuration. In ipv6AccessConfigs, the recommended name is External IPv6.</rdfs:comment>
    <rdfs:domain rdf:resource="http://example.org/onto/class/google_compute_instance_from_template"/>
    <rdfs:range rdf:resource="http://www.w3.org/2001/XMLSchema#string"/>
  </owl:DatatypeProperty>
  <owl:DatatypeProperty rdf:about="http://example.org/onto/prop/google_compute_instance_from_template_network_tier">
    <rdfs:label>network_tier</rdfs:label>
    <rdfs:comment>The service-level to be provided for IPv6 traffic when the subnet has an external subnet. Only PREMIUM tier is valid for IPv6</rdfs:comment>
    <rdfs:domain rdf:resource="http://example.org/onto/class/google_compute_instance_from_template"/>
    <rdfs:range rdf:resource="http://www.w3.org/2001/XMLSchema#string"/>
  </owl:DatatypeProperty>
  <owl:DatatypeProperty rdf:about="http://example.org/onto/prop/google_compute_instance_from_template_public_ptr_domain_name">
    <rdfs:label>public_ptr_domain_name</rdfs:label>
    <rdfs:comment>The domain name to be used when creating DNSv6 records for the external IPv6 ranges.</rdfs:comment>
    <rdfs:domain rdf:resource="http://example.org/onto/class/google_compute_instance_from_template"/>
    <rdfs:range rdf:resource="http://www.w3.org/2001/XMLSchema#string"/>
  </owl:DatatypeProperty>
  <owl:DatatypeProperty rdf:about="http://example.org/onto/prop/google_compute_instance_from_template_total_egress_bandwidth_tier">
    <rdfs:label>total_egress_bandwidth_tier</rdfs:label>
    <rdfs:comment>The egress bandwidth tier to enable. Possible values:TIER_1, DEFAULT</rdfs:comment>
    <rdfs:domain rdf:resource="http://example.org/onto/class/google_compute_instance_from_template"/>
    <rdfs:range rdf:resource="http://www.w3.org/2001/XMLSchema#string"/>
  </owl:DatatypeProperty>
  <owl:DatatypeProperty rdf:about="http://example.org/onto/prop/google_compute_instance_from_template_resource_manager_tags">
    <rdfs:label>resource_manager_tags</rdfs:label>
    <rdfs:comment>A map of resource manager tags. Resource manager tag keys and values have the same definition as resource manager tags. Keys must be in the format tagKeys/{tag_key_id}, and values are in the format tagValues/456. The field is ignored (both PUT & PATCH) when empty.</rdfs:comment>
    <rdfs:domain rdf:resource="http://example.org/onto/class/google_compute_instance_from_template"/>
    <rdfs:range rdf:resource="http://www.w3.org/2001/XMLSchema#string"/>
  </owl:DatatypeProperty>
  <owl:DatatypeProperty rdf:about="http://example.org/onto/prop/google_compute_instance_from_template_type">
    <rdfs:label>type</rdfs:label>
    <rdfs:comment>The type of reservation from which this instance can consume resources.</rdfs:comment>
    <rdfs:domain rdf:resource="http://example.org/onto/class/google_compute_instance_from_template"/>
    <rdfs:range rdf:resource="http://www.w3.org/2001/XMLSchema#string"/>
  </owl:DatatypeProperty>
  <owl:DatatypeProperty rdf:about="http://example.org/onto/prop/google_compute_instance_from_template_key">
    <rdfs:label>key</rdfs:label>
    <rdfs:comment>Corresponds to the label key of a reservation resource. To target a SPECIFIC_RESERVATION by name, specify compute.googleapis.com/reservation-name as the key and specify the name of your reservation as the only value.</rdfs:comment>
    <rdfs:domain rdf:resource="http://example.org/onto/class/google_compute_instance_from_template"/>
    <rdfs:range rdf:resource="http://www.w3.org/2001/XMLSchema#string"/>
  </owl:DatatypeProperty>
  <owl:DatatypeProperty rdf:about="http://example.org/onto/prop/google_compute_instance_from_template_values">
    <rdfs:label>values</rdfs:label>
    <rdfs:comment>Corresponds to the label values of a reservation resource.</rdfs:comment>
    <rdfs:domain rdf:resource="http://example.org/onto/class/google_compute_instance_from_template"/>
    <rdfs:range rdf:resource="http://www.w3.org/2001/XMLSchema#string"/>
  </owl:DatatypeProperty>
  <owl:DatatypeProperty rdf:about="http://example.org/onto/prop/google_compute_instance_from_template_automatic_restart">
    <rdfs:label>automatic_restart</rdfs:label>
    <rdfs:comment>Specifies if the instance should be restarted if it was terminated by Compute Engine (not a user).</rdfs:comment>
    <rdfs:domain rdf:resource="http://example.org/onto/class/google_compute_instance_from_template"/>
    <rdfs:range rdf:resource="http://www.w3.org/2001/XMLSchema#string"/>
  </owl:DatatypeProperty>
  <owl:DatatypeProperty rdf:about="http://example.org/onto/prop/google_compute_instance_from_template_availability_domain">
    <rdfs:label>availability_domain</rdfs:label>
    <rdfs:comment>Specifies the availability domain, which this instance should be scheduled on.</rdfs:comment>
    <rdfs:domain rdf:resource="http://example.org/onto/class/google_compute_instance_from_template"/>
    <rdfs:range rdf:resource="http://www.w3.org/2001/XMLSchema#string"/>
  </owl:DatatypeProperty>
  <owl:DatatypeProperty rdf:about="http://example.org/onto/prop/google_compute_instance_from_template_instance_termination_action">
    <rdfs:label>instance_termination_action</rdfs:label>
    <rdfs:comment>Specifies the action GCE should take when SPOT VM is preempted.</rdfs:comment>
    <rdfs:domain rdf:resource="http://example.org/onto/class/google_compute_instance_from_template"/>
    <rdfs:range rdf:resource="http://www.w3.org/2001/XMLSchema#string"/>
  </owl:DatatypeProperty>
  <owl:DatatypeProperty rdf:about="http://example.org/onto/prop/google_compute_instance_from_template_min_node_cpus">
    <rdfs:label>min_node_cpus</rdfs:label>
    <rdfs:domain rdf:resource="http://example.org/onto/class/google_compute_instance_from_template"/>
    <rdfs:range rdf:resource="http://www.w3.org/2001/XMLSchema#string"/>
  </owl:DatatypeProperty>
  <owl:DatatypeProperty rdf:about="http://example.org/onto/prop/google_compute_instance_from_template_on_host_maintenance">
    <rdfs:label>on_host_maintenance</rdfs:label>
    <rdfs:comment>Describes maintenance behavior for the instance. One of MIGRATE or TERMINATE,</rdfs:comment>
    <rdfs:domain rdf:resource="http://example.org/onto/class/google_compute_instance_from_template"/>
    <rdfs:range rdf:resource="http://www.w3.org/2001/XMLSchema#string"/>
  </owl:DatatypeProperty>
  <owl:DatatypeProperty rdf:about="http://example.org/onto/prop/google_compute_instance_from_template_preemptible">
    <rdfs:label>preemptible</rdfs:label>
    <rdfs:comment>Whether the instance is preemptible.</rdfs:comment>
    <rdfs:domain rdf:resource="http://example.org/onto/class/google_compute_instance_from_template"/>
    <rdfs:range rdf:resource="http://www.w3.org/2001/XMLSchema#string"/>
  </owl:DatatypeProperty>
  <owl:DatatypeProperty rdf:about="http://example.org/onto/prop/google_compute_instance_from_template_provisioning_model">
    <rdfs:label>provisioning_model</rdfs:label>
    <rdfs:comment>Whether the instance is spot. If this is set as SPOT.</rdfs:comment>
    <rdfs:domain rdf:resource="http://example.org/onto/class/google_compute_instance_from_template"/>
    <rdfs:range rdf:resource="http://www.w3.org/2001/XMLSchema#string"/>
  </owl:DatatypeProperty>
  <owl:DatatypeProperty rdf:about="http://example.org/onto/prop/google_compute_instance_from_template_termination_time">
    <rdfs:label>termination_time</rdfs:label>
    <rdfs:comment>Specifies the timestamp, when the instance will be terminated,
in RFC3339 text format. If specified, the instance termination action
will be performed at the termination time.</rdfs:comment>
    <rdfs:domain rdf:resource="http://example.org/onto/class/google_compute_instance_from_template"/>
    <rdfs:range rdf:resource="http://www.w3.org/2001/XMLSchema#string"/>
  </owl:DatatypeProperty>
  <owl:DatatypeProperty rdf:about="http://example.org/onto/prop/google_compute_instance_from_template_nanos">
    <rdfs:label>nanos</rdfs:label>
    <rdfs:comment>Span of time that's a fraction of a second at nanosecond
resolution. Durations less than one second are represented
with a 0 seconds field and a positive nanos field. Must
be from 0 to 999,999,999 inclusive.</rdfs:comment>
    <rdfs:domain rdf:resource="http://example.org/onto/class/google_compute_instance_from_template"/>
    <rdfs:range rdf:resource="http://www.w3.org/2001/XMLSchema#string"/>
  </owl:DatatypeProperty>
  <owl:DatatypeProperty rdf:about="http://example.org/onto/prop/google_compute_instance_from_template_seconds">
    <rdfs:label>seconds</rdfs:label>
    <rdfs:comment>Span of time at a resolution of a second.
Must be from 0 to 315,576,000,000 inclusive.</rdfs:comment>
    <rdfs:domain rdf:resource="http://example.org/onto/class/google_compute_instance_from_template"/>
    <rdfs:range rdf:resource="http://www.w3.org/2001/XMLSchema#string"/>
  </owl:DatatypeProperty>
  <owl:DatatypeProperty rdf:about="http://example.org/onto/prop/google_compute_instance_from_template_nanos">
    <rdfs:label>nanos</rdfs:label>
    <rdfs:comment>Span of time that's a fraction of a second at nanosecond
resolution. Durations less than one second are represented
with a 0 seconds field and a positive nanos field. Must
be from 0 to 999,999,999 inclusive.</rdfs:comment>
    <rdfs:domain rdf:resource="http://example.org/onto/class/google_compute_instance_from_template"/>
    <rdfs:range rdf:resource="http://www.w3.org/2001/XMLSchema#string"/>
  </owl:DatatypeProperty>
  <owl:DatatypeProperty rdf:about="http://example.org/onto/prop/google_compute_instance_from_template_seconds">
    <rdfs:label>seconds</rdfs:label>
    <rdfs:comment>Span of time at a resolution of a second.
Must be from 0 to 315,576,000,000 inclusive.</rdfs:comment>
    <rdfs:domain rdf:resource="http://example.org/onto/class/google_compute_instance_from_template"/>
    <rdfs:range rdf:resource="http://www.w3.org/2001/XMLSchema#string"/>
  </owl:DatatypeProperty>
  <owl:DatatypeProperty rdf:about="http://example.org/onto/prop/google_compute_instance_from_template_key">
    <rdfs:label>key</rdfs:label>
    <rdfs:domain rdf:resource="http://example.org/onto/class/google_compute_instance_from_template"/>
    <rdfs:range rdf:resource="http://www.w3.org/2001/XMLSchema#string"/>
  </owl:DatatypeProperty>
  <owl:DatatypeProperty rdf:about="http://example.org/onto/prop/google_compute_instance_from_template_operator">
    <rdfs:label>operator</rdfs:label>
    <rdfs:domain rdf:resource="http://example.org/onto/class/google_compute_instance_from_template"/>
    <rdfs:range rdf:resource="http://www.w3.org/2001/XMLSchema#string"/>
  </owl:DatatypeProperty>
  <owl:DatatypeProperty rdf:about="http://example.org/onto/prop/google_compute_instance_from_template_values">
    <rdfs:label>values</rdfs:label>
    <rdfs:domain rdf:resource="http://example.org/onto/class/google_compute_instance_from_template"/>
    <rdfs:range rdf:resource="http://www.w3.org/2001/XMLSchema#string"/>
  </owl:DatatypeProperty>
  <owl:DatatypeProperty rdf:about="http://example.org/onto/prop/google_compute_instance_from_template_discard_local_ssd">
    <rdfs:label>discard_local_ssd</rdfs:label>
    <rdfs:comment>If true, the contents of any attached Local SSD disks will be discarded.</rdfs:comment>
    <rdfs:domain rdf:resource="http://example.org/onto/class/google_compute_instance_from_template"/>
    <rdfs:range rdf:resource="http://www.w3.org/2001/XMLSchema#string"/>
  </owl:DatatypeProperty>
  <owl:DatatypeProperty rdf:about="http://example.org/onto/prop/google_compute_instance_from_template_device_name">
    <rdfs:label>device_name</rdfs:label>
    <rdfs:comment>Name with which the attached disk is accessible under /dev/disk/by-id/</rdfs:comment>
    <rdfs:domain rdf:resource="http://example.org/onto/class/google_compute_instance_from_template"/>
    <rdfs:range rdf:resource="http://www.w3.org/2001/XMLSchema#string"/>
  </owl:DatatypeProperty>
  <owl:DatatypeProperty rdf:about="http://example.org/onto/prop/google_compute_instance_from_template_interface">
    <rdfs:label>interface</rdfs:label>
    <rdfs:comment>The disk interface used for attaching this disk. One of SCSI or NVME.</rdfs:comment>
    <rdfs:domain rdf:resource="http://example.org/onto/class/google_compute_instance_from_template"/>
    <rdfs:range rdf:resource="http://www.w3.org/2001/XMLSchema#string"/>
  </owl:DatatypeProperty>
  <owl:DatatypeProperty rdf:about="http://example.org/onto/prop/google_compute_instance_from_template_size">
    <rdfs:label>size</rdfs:label>
    <rdfs:comment>The size of the disk in gigabytes. One of 375 or 3000.</rdfs:comment>
    <rdfs:domain rdf:resource="http://example.org/onto/class/google_compute_instance_from_template"/>
    <rdfs:range rdf:resource="http://www.w3.org/2001/XMLSchema#string"/>
  </owl:DatatypeProperty>
  <owl:DatatypeProperty rdf:about="http://example.org/onto/prop/google_compute_instance_from_template_email">
    <rdfs:label>email</rdfs:label>
    <rdfs:comment>The service account e-mail address.</rdfs:comment>
    <rdfs:domain rdf:resource="http://example.org/onto/class/google_compute_instance_from_template"/>
    <rdfs:range rdf:resource="http://www.w3.org/2001/XMLSchema#string"/>
  </owl:DatatypeProperty>
  <owl:DatatypeProperty rdf:about="http://example.org/onto/prop/google_compute_instance_from_template_scopes">
    <rdfs:label>scopes</rdfs:label>
    <rdfs:comment>A list of service scopes.</rdfs:comment>
    <rdfs:domain rdf:resource="http://example.org/onto/class/google_compute_instance_from_template"/>
    <rdfs:range rdf:resource="http://www.w3.org/2001/XMLSchema#string"/>
  </owl:DatatypeProperty>
  <owl:DatatypeProperty rdf:about="http://example.org/onto/prop/google_compute_instance_from_template_enable_integrity_monitoring">
    <rdfs:label>enable_integrity_monitoring</rdfs:label>
    <rdfs:comment>Whether integrity monitoring is enabled for the instance.</rdfs:comment>
    <rdfs:domain rdf:resource="http://example.org/onto/class/google_compute_instance_from_template"/>
    <rdfs:range rdf:resource="http://www.w3.org/2001/XMLSchema#string"/>
  </owl:DatatypeProperty>
  <owl:DatatypeProperty rdf:about="http://example.org/onto/prop/google_compute_instance_from_template_enable_secure_boot">
    <rdfs:label>enable_secure_boot</rdfs:label>
    <rdfs:comment>Whether secure boot is enabled for the instance.</rdfs:comment>
    <rdfs:domain rdf:resource="http://example.org/onto/class/google_compute_instance_from_template"/>
    <rdfs:range rdf:resource="http://www.w3.org/2001/XMLSchema#string"/>
  </owl:DatatypeProperty>
  <owl:DatatypeProperty rdf:about="http://example.org/onto/prop/google_compute_instance_from_template_enable_vtpm">
    <rdfs:label>enable_vtpm</rdfs:label>
    <rdfs:comment>Whether the instance uses vTPM.</rdfs:comment>
    <rdfs:domain rdf:resource="http://example.org/onto/class/google_compute_instance_from_template"/>
    <rdfs:range rdf:resource="http://www.w3.org/2001/XMLSchema#string"/>
  </owl:DatatypeProperty>
  <owl:DatatypeProperty rdf:about="http://example.org/onto/prop/google_compute_instance_from_template_create">
    <rdfs:label>create</rdfs:label>
    <rdfs:domain rdf:resource="http://example.org/onto/class/google_compute_instance_from_template"/>
    <rdfs:range rdf:resource="http://www.w3.org/2001/XMLSchema#string"/>
  </owl:DatatypeProperty>
  <owl:DatatypeProperty rdf:about="http://example.org/onto/prop/google_compute_instance_from_template_delete">
    <rdfs:label>delete</rdfs:label>
    <rdfs:domain rdf:resource="http://example.org/onto/class/google_compute_instance_from_template"/>
    <rdfs:range rdf:resource="http://www.w3.org/2001/XMLSchema#string"/>
  </owl:DatatypeProperty>
  <owl:DatatypeProperty rdf:about="http://example.org/onto/prop/google_compute_instance_from_template_update">
    <rdfs:label>update</rdfs:label>
    <rdfs:domain rdf:resource="http://example.org/onto/class/google_compute_instance_from_template"/>
    <rdfs:range rdf:resource="http://www.w3.org/2001/XMLSchema#string"/>
  </owl:DatatypeProperty>
</rdf:RDF>
