<?xml version="1.0" encoding="UTF-8"?>
<rdf:RDF
  xmlns:rdf="http://www.w3.org/1999/02/22-rdf-syntax-ns#"
  xmlns:rdfs="http://www.w3.org/2000/01/rdf-schema#"
  xmlns:owl="http://www.w3.org/2002/07/owl#"
  xmlns:xsd="http://www.w3.org/2001/XMLSchema#"
  xml:base="http://example.org/onto/">
  <owl:Class rdf:about="http://example.org/onto/class/google_cloud_scheduler_job">
    <rdfs:label>google_cloud_scheduler_job</rdfs:label>
    <rdfs:comment>#
#     ***     AUTO GENERATED CODE    ***    Type: MMv1     ***
#
# ----------------------------------------------------------------------------
#
#     This code is generated by Magic Modules using the following:
#
#     Configuration: https:#github.com/GoogleCloudPlatform/magic-modules/tree/main/mmv1/products/cloudscheduler/Job.yaml
#     Template:      https:#github.com/GoogleCloudPlatform/magic-modules/tree/main/mmv1/templates/terraform/resource.html.markdown.tmpl
#
#     DO NOT EDIT this file directly. Any changes made to this file will be
#     overwritten during the next generation cycle.
#
# ----------------------------------------------------------------------------
subcategory: "Cloud Scheduler"
description: |-
  A scheduled job that can publish a PubSub message or an HTTP request
  every X interval of time, using a crontab format string.
---</rdfs:comment>
  </owl:Class>
  <owl:DatatypeProperty rdf:about="http://example.org/onto/prop/google_cloud_scheduler_job_attempt_deadline">
    <rdfs:label>attempt_deadline</rdfs:label>
    <rdfs:comment>The deadline for job attempts. If the request handler does not respond by this deadline then the request is
cancelled and the attempt is marked as a DEADLINE_EXCEEDED failure. The failed attempt can be viewed in
execution logs. Cloud Scheduler will retry the job according to the RetryConfig.
The allowed duration for this deadline is:
* For HTTP targets, between 15 seconds and 30 minutes.
* For App Engine HTTP targets, between 15 seconds and 24 hours.
* **Note**: For PubSub targets, this field is ignored - setting it will introduce an unresolvable diff.
A duration in seconds with up to nine fractional digits, terminated by 's'. Example: "3.5s"</rdfs:comment>
    <rdfs:domain rdf:resource="http://example.org/onto/class/google_cloud_scheduler_job"/>
    <rdfs:range rdf:resource="http://www.w3.org/2001/XMLSchema#string"/>
  </owl:DatatypeProperty>
  <owl:DatatypeProperty rdf:about="http://example.org/onto/prop/google_cloud_scheduler_job_description">
    <rdfs:label>description</rdfs:label>
    <rdfs:comment>A human-readable description for the job.
This string must not contain more than 500 characters.</rdfs:comment>
    <rdfs:domain rdf:resource="http://example.org/onto/class/google_cloud_scheduler_job"/>
    <rdfs:range rdf:resource="http://www.w3.org/2001/XMLSchema#string"/>
  </owl:DatatypeProperty>
  <owl:DatatypeProperty rdf:about="http://example.org/onto/prop/google_cloud_scheduler_job_id">
    <rdfs:label>id</rdfs:label>
    <rdfs:domain rdf:resource="http://example.org/onto/class/google_cloud_scheduler_job"/>
    <rdfs:range rdf:resource="http://www.w3.org/2001/XMLSchema#string"/>
  </owl:DatatypeProperty>
  <owl:DatatypeProperty rdf:about="http://example.org/onto/prop/google_cloud_scheduler_job_name">
    <rdfs:label>name</rdfs:label>
    <rdfs:comment>The name of the job.</rdfs:comment>
    <rdfs:domain rdf:resource="http://example.org/onto/class/google_cloud_scheduler_job"/>
    <rdfs:range rdf:resource="http://www.w3.org/2001/XMLSchema#string"/>
  </owl:DatatypeProperty>
  <owl:DatatypeProperty rdf:about="http://example.org/onto/prop/google_cloud_scheduler_job_paused">
    <rdfs:label>paused</rdfs:label>
    <rdfs:comment>Sets the job to a paused state. Jobs default to being enabled when this property is not set.</rdfs:comment>
    <rdfs:domain rdf:resource="http://example.org/onto/class/google_cloud_scheduler_job"/>
    <rdfs:range rdf:resource="http://www.w3.org/2001/XMLSchema#string"/>
  </owl:DatatypeProperty>
  <owl:DatatypeProperty rdf:about="http://example.org/onto/prop/google_cloud_scheduler_job_project">
    <rdfs:label>project</rdfs:label>
    <rdfs:domain rdf:resource="http://example.org/onto/class/google_cloud_scheduler_job"/>
    <rdfs:range rdf:resource="http://www.w3.org/2001/XMLSchema#string"/>
  </owl:DatatypeProperty>
  <owl:DatatypeProperty rdf:about="http://example.org/onto/prop/google_cloud_scheduler_job_region">
    <rdfs:label>region</rdfs:label>
    <rdfs:comment>Region where the scheduler job resides. If it is not provided, Terraform will use the provider default.</rdfs:comment>
    <rdfs:domain rdf:resource="http://example.org/onto/class/google_cloud_scheduler_job"/>
    <rdfs:range rdf:resource="http://www.w3.org/2001/XMLSchema#string"/>
  </owl:DatatypeProperty>
  <owl:DatatypeProperty rdf:about="http://example.org/onto/prop/google_cloud_scheduler_job_schedule">
    <rdfs:label>schedule</rdfs:label>
    <rdfs:comment>Describes the schedule on which the job will be executed.</rdfs:comment>
    <rdfs:domain rdf:resource="http://example.org/onto/class/google_cloud_scheduler_job"/>
    <rdfs:range rdf:resource="http://www.w3.org/2001/XMLSchema#string"/>
  </owl:DatatypeProperty>
  <owl:DatatypeProperty rdf:about="http://example.org/onto/prop/google_cloud_scheduler_job_state">
    <rdfs:label>state</rdfs:label>
    <rdfs:comment>State of the job.</rdfs:comment>
    <rdfs:domain rdf:resource="http://example.org/onto/class/google_cloud_scheduler_job"/>
    <rdfs:range rdf:resource="http://www.w3.org/2001/XMLSchema#string"/>
  </owl:DatatypeProperty>
  <owl:DatatypeProperty rdf:about="http://example.org/onto/prop/google_cloud_scheduler_job_time_zone">
    <rdfs:label>time_zone</rdfs:label>
    <rdfs:comment>Specifies the time zone to be used in interpreting schedule.
The value of this field must be a time zone name from the tz database.</rdfs:comment>
    <rdfs:domain rdf:resource="http://example.org/onto/class/google_cloud_scheduler_job"/>
    <rdfs:range rdf:resource="http://www.w3.org/2001/XMLSchema#string"/>
  </owl:DatatypeProperty>
  <owl:DatatypeProperty rdf:about="http://example.org/onto/prop/google_cloud_scheduler_job_body">
    <rdfs:label>body</rdfs:label>
    <rdfs:comment>HTTP request body.
A request body is allowed only if the HTTP method is POST or PUT.
It will result in invalid argument error to set a body on a job with an incompatible HttpMethod.

A base64-encoded string.</rdfs:comment>
    <rdfs:domain rdf:resource="http://example.org/onto/class/google_cloud_scheduler_job"/>
    <rdfs:range rdf:resource="http://www.w3.org/2001/XMLSchema#string"/>
  </owl:DatatypeProperty>
  <owl:DatatypeProperty rdf:about="http://example.org/onto/prop/google_cloud_scheduler_job_headers">
    <rdfs:label>headers</rdfs:label>
    <rdfs:comment>HTTP request headers.
This map contains the header field names and values.
Headers can be set when the job is created.</rdfs:comment>
    <rdfs:domain rdf:resource="http://example.org/onto/class/google_cloud_scheduler_job"/>
    <rdfs:range rdf:resource="http://www.w3.org/2001/XMLSchema#string"/>
  </owl:DatatypeProperty>
  <owl:DatatypeProperty rdf:about="http://example.org/onto/prop/google_cloud_scheduler_job_http_method">
    <rdfs:label>http_method</rdfs:label>
    <rdfs:comment>Which HTTP method to use for the request.</rdfs:comment>
    <rdfs:domain rdf:resource="http://example.org/onto/class/google_cloud_scheduler_job"/>
    <rdfs:range rdf:resource="http://www.w3.org/2001/XMLSchema#string"/>
  </owl:DatatypeProperty>
  <owl:DatatypeProperty rdf:about="http://example.org/onto/prop/google_cloud_scheduler_job_relative_uri">
    <rdfs:label>relative_uri</rdfs:label>
    <rdfs:comment>The relative URI.
The relative URL must begin with "/" and must be a valid HTTP relative URL.
It can contain a path, query string arguments, and \# fragments.
If the relative URL is empty, then the root path "/" will be used.
No spaces are allowed, and the maximum length allowed is 2083 characters</rdfs:comment>
    <rdfs:domain rdf:resource="http://example.org/onto/class/google_cloud_scheduler_job"/>
    <rdfs:range rdf:resource="http://www.w3.org/2001/XMLSchema#string"/>
  </owl:DatatypeProperty>
  <owl:DatatypeProperty rdf:about="http://example.org/onto/prop/google_cloud_scheduler_job_instance">
    <rdfs:label>instance</rdfs:label>
    <rdfs:comment>App instance.
By default, the job is sent to an instance which is available when the job is attempted.</rdfs:comment>
    <rdfs:domain rdf:resource="http://example.org/onto/class/google_cloud_scheduler_job"/>
    <rdfs:range rdf:resource="http://www.w3.org/2001/XMLSchema#string"/>
  </owl:DatatypeProperty>
  <owl:DatatypeProperty rdf:about="http://example.org/onto/prop/google_cloud_scheduler_job_service">
    <rdfs:label>service</rdfs:label>
    <rdfs:comment>App service.
By default, the job is sent to the service which is the default service when the job is attempted.</rdfs:comment>
    <rdfs:domain rdf:resource="http://example.org/onto/class/google_cloud_scheduler_job"/>
    <rdfs:range rdf:resource="http://www.w3.org/2001/XMLSchema#string"/>
  </owl:DatatypeProperty>
  <owl:DatatypeProperty rdf:about="http://example.org/onto/prop/google_cloud_scheduler_job_version">
    <rdfs:label>version</rdfs:label>
    <rdfs:comment>App version.
By default, the job is sent to the version which is the default version when the job is attempted.</rdfs:comment>
    <rdfs:domain rdf:resource="http://example.org/onto/class/google_cloud_scheduler_job"/>
    <rdfs:range rdf:resource="http://www.w3.org/2001/XMLSchema#string"/>
  </owl:DatatypeProperty>
  <owl:DatatypeProperty rdf:about="http://example.org/onto/prop/google_cloud_scheduler_job_body">
    <rdfs:label>body</rdfs:label>
    <rdfs:comment>HTTP request body.
A request body is allowed only if the HTTP method is POST, PUT, or PATCH.
It is an error to set body on a job with an incompatible HttpMethod.

A base64-encoded string.</rdfs:comment>
    <rdfs:domain rdf:resource="http://example.org/onto/class/google_cloud_scheduler_job"/>
    <rdfs:range rdf:resource="http://www.w3.org/2001/XMLSchema#string"/>
  </owl:DatatypeProperty>
  <owl:DatatypeProperty rdf:about="http://example.org/onto/prop/google_cloud_scheduler_job_headers">
    <rdfs:label>headers</rdfs:label>
    <rdfs:comment>This map contains the header field names and values.
Repeated headers are not supported, but a header value can contain commas.</rdfs:comment>
    <rdfs:domain rdf:resource="http://example.org/onto/class/google_cloud_scheduler_job"/>
    <rdfs:range rdf:resource="http://www.w3.org/2001/XMLSchema#string"/>
  </owl:DatatypeProperty>
  <owl:DatatypeProperty rdf:about="http://example.org/onto/prop/google_cloud_scheduler_job_http_method">
    <rdfs:label>http_method</rdfs:label>
    <rdfs:comment>Which HTTP method to use for the request.</rdfs:comment>
    <rdfs:domain rdf:resource="http://example.org/onto/class/google_cloud_scheduler_job"/>
    <rdfs:range rdf:resource="http://www.w3.org/2001/XMLSchema#string"/>
  </owl:DatatypeProperty>
  <owl:DatatypeProperty rdf:about="http://example.org/onto/prop/google_cloud_scheduler_job_uri">
    <rdfs:label>uri</rdfs:label>
    <rdfs:comment>The full URI path that the request will be sent to.</rdfs:comment>
    <rdfs:domain rdf:resource="http://example.org/onto/class/google_cloud_scheduler_job"/>
    <rdfs:range rdf:resource="http://www.w3.org/2001/XMLSchema#string"/>
  </owl:DatatypeProperty>
  <owl:DatatypeProperty rdf:about="http://example.org/onto/prop/google_cloud_scheduler_job_scope">
    <rdfs:label>scope</rdfs:label>
    <rdfs:comment>OAuth scope to be used for generating OAuth access token. If not specified,
"https://www.googleapis.com/auth/cloud-platform" will be used.</rdfs:comment>
    <rdfs:domain rdf:resource="http://example.org/onto/class/google_cloud_scheduler_job"/>
    <rdfs:range rdf:resource="http://www.w3.org/2001/XMLSchema#string"/>
  </owl:DatatypeProperty>
  <owl:DatatypeProperty rdf:about="http://example.org/onto/prop/google_cloud_scheduler_job_service_account_email">
    <rdfs:label>service_account_email</rdfs:label>
    <rdfs:comment>Service account email to be used for generating OAuth token.
The service account must be within the same project as the job.</rdfs:comment>
    <rdfs:domain rdf:resource="http://example.org/onto/class/google_cloud_scheduler_job"/>
    <rdfs:range rdf:resource="http://www.w3.org/2001/XMLSchema#string"/>
  </owl:DatatypeProperty>
  <owl:DatatypeProperty rdf:about="http://example.org/onto/prop/google_cloud_scheduler_job_audience">
    <rdfs:label>audience</rdfs:label>
    <rdfs:comment>Audience to be used when generating OIDC token. If not specified,
the URI specified in target will be used.</rdfs:comment>
    <rdfs:domain rdf:resource="http://example.org/onto/class/google_cloud_scheduler_job"/>
    <rdfs:range rdf:resource="http://www.w3.org/2001/XMLSchema#string"/>
  </owl:DatatypeProperty>
  <owl:DatatypeProperty rdf:about="http://example.org/onto/prop/google_cloud_scheduler_job_service_account_email">
    <rdfs:label>service_account_email</rdfs:label>
    <rdfs:comment>Service account email to be used for generating OAuth token.
The service account must be within the same project as the job.</rdfs:comment>
    <rdfs:domain rdf:resource="http://example.org/onto/class/google_cloud_scheduler_job"/>
    <rdfs:range rdf:resource="http://www.w3.org/2001/XMLSchema#string"/>
  </owl:DatatypeProperty>
  <owl:DatatypeProperty rdf:about="http://example.org/onto/prop/google_cloud_scheduler_job_attributes">
    <rdfs:label>attributes</rdfs:label>
    <rdfs:comment>Attributes for PubsubMessage.
Pubsub message must contain either non-empty data, or at least one attribute.</rdfs:comment>
    <rdfs:domain rdf:resource="http://example.org/onto/class/google_cloud_scheduler_job"/>
    <rdfs:range rdf:resource="http://www.w3.org/2001/XMLSchema#string"/>
  </owl:DatatypeProperty>
  <owl:DatatypeProperty rdf:about="http://example.org/onto/prop/google_cloud_scheduler_job_data">
    <rdfs:label>data</rdfs:label>
    <rdfs:comment>The message payload for PubsubMessage.
Pubsub message must contain either non-empty data, or at least one attribute.

 A base64-encoded string.</rdfs:comment>
    <rdfs:domain rdf:resource="http://example.org/onto/class/google_cloud_scheduler_job"/>
    <rdfs:range rdf:resource="http://www.w3.org/2001/XMLSchema#string"/>
  </owl:DatatypeProperty>
  <owl:DatatypeProperty rdf:about="http://example.org/onto/prop/google_cloud_scheduler_job_topic_name">
    <rdfs:label>topic_name</rdfs:label>
    <rdfs:comment>The full resource name for the Cloud Pub/Sub topic to which
messages will be published when a job is delivered. ~>**NOTE:**
The topic name must be in the same format as required by PubSub's
PublishRequest.name, e.g. 'projects/my-project/topics/my-topic'.</rdfs:comment>
    <rdfs:domain rdf:resource="http://example.org/onto/class/google_cloud_scheduler_job"/>
    <rdfs:range rdf:resource="http://www.w3.org/2001/XMLSchema#string"/>
  </owl:DatatypeProperty>
  <owl:DatatypeProperty rdf:about="http://example.org/onto/prop/google_cloud_scheduler_job_max_backoff_duration">
    <rdfs:label>max_backoff_duration</rdfs:label>
    <rdfs:comment>The maximum amount of time to wait before retrying a job after it fails.
A duration in seconds with up to nine fractional digits, terminated by 's'.</rdfs:comment>
    <rdfs:domain rdf:resource="http://example.org/onto/class/google_cloud_scheduler_job"/>
    <rdfs:range rdf:resource="http://www.w3.org/2001/XMLSchema#string"/>
  </owl:DatatypeProperty>
  <owl:DatatypeProperty rdf:about="http://example.org/onto/prop/google_cloud_scheduler_job_max_doublings">
    <rdfs:label>max_doublings</rdfs:label>
    <rdfs:comment>The time between retries will double maxDoublings times.
A job's retry interval starts at minBackoffDuration,
then doubles maxDoublings times, then increases linearly,
and finally retries retries at intervals of maxBackoffDuration up to retryCount times.</rdfs:comment>
    <rdfs:domain rdf:resource="http://example.org/onto/class/google_cloud_scheduler_job"/>
    <rdfs:range rdf:resource="http://www.w3.org/2001/XMLSchema#string"/>
  </owl:DatatypeProperty>
  <owl:DatatypeProperty rdf:about="http://example.org/onto/prop/google_cloud_scheduler_job_max_retry_duration">
    <rdfs:label>max_retry_duration</rdfs:label>
    <rdfs:comment>The time limit for retrying a failed job, measured from time when an execution was first attempted.
If specified with retryCount, the job will be retried until both limits are reached.
A duration in seconds with up to nine fractional digits, terminated by 's'.</rdfs:comment>
    <rdfs:domain rdf:resource="http://example.org/onto/class/google_cloud_scheduler_job"/>
    <rdfs:range rdf:resource="http://www.w3.org/2001/XMLSchema#string"/>
  </owl:DatatypeProperty>
  <owl:DatatypeProperty rdf:about="http://example.org/onto/prop/google_cloud_scheduler_job_min_backoff_duration">
    <rdfs:label>min_backoff_duration</rdfs:label>
    <rdfs:comment>The minimum amount of time to wait before retrying a job after it fails.
A duration in seconds with up to nine fractional digits, terminated by 's'.</rdfs:comment>
    <rdfs:domain rdf:resource="http://example.org/onto/class/google_cloud_scheduler_job"/>
    <rdfs:range rdf:resource="http://www.w3.org/2001/XMLSchema#string"/>
  </owl:DatatypeProperty>
  <owl:DatatypeProperty rdf:about="http://example.org/onto/prop/google_cloud_scheduler_job_retry_count">
    <rdfs:label>retry_count</rdfs:label>
    <rdfs:comment>The number of attempts that the system will make to run a
job using the exponential backoff procedure described by maxDoublings.
Values greater than 5 and negative values are not allowed.</rdfs:comment>
    <rdfs:domain rdf:resource="http://example.org/onto/class/google_cloud_scheduler_job"/>
    <rdfs:range rdf:resource="http://www.w3.org/2001/XMLSchema#string"/>
  </owl:DatatypeProperty>
  <owl:DatatypeProperty rdf:about="http://example.org/onto/prop/google_cloud_scheduler_job_create">
    <rdfs:label>create</rdfs:label>
    <rdfs:domain rdf:resource="http://example.org/onto/class/google_cloud_scheduler_job"/>
    <rdfs:range rdf:resource="http://www.w3.org/2001/XMLSchema#string"/>
  </owl:DatatypeProperty>
  <owl:DatatypeProperty rdf:about="http://example.org/onto/prop/google_cloud_scheduler_job_delete">
    <rdfs:label>delete</rdfs:label>
    <rdfs:domain rdf:resource="http://example.org/onto/class/google_cloud_scheduler_job"/>
    <rdfs:range rdf:resource="http://www.w3.org/2001/XMLSchema#string"/>
  </owl:DatatypeProperty>
  <owl:DatatypeProperty rdf:about="http://example.org/onto/prop/google_cloud_scheduler_job_update">
    <rdfs:label>update</rdfs:label>
    <rdfs:domain rdf:resource="http://example.org/onto/class/google_cloud_scheduler_job"/>
    <rdfs:range rdf:resource="http://www.w3.org/2001/XMLSchema#string"/>
  </owl:DatatypeProperty>
</rdf:RDF>
