<?xml version="1.0" encoding="UTF-8"?>
<rdf:RDF
  xmlns:rdf="http://www.w3.org/1999/02/22-rdf-syntax-ns#"
  xmlns:rdfs="http://www.w3.org/2000/01/rdf-schema#"
  xmlns:owl="http://www.w3.org/2002/07/owl#"
  xmlns:xsd="http://www.w3.org/2001/XMLSchema#"
  xml:base="http://example.org/onto/">
  <owl:Class rdf:about="http://example.org/onto/class/google_data_loss_prevention_inspect_template">
    <rdfs:label>google_data_loss_prevention_inspect_template</rdfs:label>
    <rdfs:comment>#
#     ***     AUTO GENERATED CODE    ***    Type: MMv1     ***
#
# ----------------------------------------------------------------------------
#
#     This code is generated by Magic Modules using the following:
#
#     Configuration: https:#github.com/GoogleCloudPlatform/magic-modules/tree/main/mmv1/products/dlp/InspectTemplate.yaml
#     Template:      https:#github.com/GoogleCloudPlatform/magic-modules/tree/main/mmv1/templates/terraform/resource.html.markdown.tmpl
#
#     DO NOT EDIT this file directly. Any changes made to this file will be
#     overwritten during the next generation cycle.
#
# ----------------------------------------------------------------------------
subcategory: "Data Loss Prevention"
description: |-
  An inspect job template.
---</rdfs:comment>
  </owl:Class>
  <owl:DatatypeProperty rdf:about="http://example.org/onto/prop/google_data_loss_prevention_inspect_template_description">
    <rdfs:label>description</rdfs:label>
    <rdfs:comment>A description of the inspect template.</rdfs:comment>
    <rdfs:domain rdf:resource="http://example.org/onto/class/google_data_loss_prevention_inspect_template"/>
    <rdfs:range rdf:resource="http://www.w3.org/2001/XMLSchema#string"/>
  </owl:DatatypeProperty>
  <owl:DatatypeProperty rdf:about="http://example.org/onto/prop/google_data_loss_prevention_inspect_template_display_name">
    <rdfs:label>display_name</rdfs:label>
    <rdfs:comment>User set display name of the inspect template.</rdfs:comment>
    <rdfs:domain rdf:resource="http://example.org/onto/class/google_data_loss_prevention_inspect_template"/>
    <rdfs:range rdf:resource="http://www.w3.org/2001/XMLSchema#string"/>
  </owl:DatatypeProperty>
  <owl:DatatypeProperty rdf:about="http://example.org/onto/prop/google_data_loss_prevention_inspect_template_id">
    <rdfs:label>id</rdfs:label>
    <rdfs:domain rdf:resource="http://example.org/onto/class/google_data_loss_prevention_inspect_template"/>
    <rdfs:range rdf:resource="http://www.w3.org/2001/XMLSchema#string"/>
  </owl:DatatypeProperty>
  <owl:DatatypeProperty rdf:about="http://example.org/onto/prop/google_data_loss_prevention_inspect_template_name">
    <rdfs:label>name</rdfs:label>
    <rdfs:comment>The resource name of the inspect template. Set by the server.</rdfs:comment>
    <rdfs:domain rdf:resource="http://example.org/onto/class/google_data_loss_prevention_inspect_template"/>
    <rdfs:range rdf:resource="http://www.w3.org/2001/XMLSchema#string"/>
  </owl:DatatypeProperty>
  <owl:DatatypeProperty rdf:about="http://example.org/onto/prop/google_data_loss_prevention_inspect_template_parent">
    <rdfs:label>parent</rdfs:label>
    <rdfs:comment>The parent of the inspect template in any of the following formats:

* 'projects/{{project}}'
* 'projects/{{project}}/locations/{{location}}'
* 'organizations/{{organization_id}}'
* 'organizations/{{organization_id}}/locations/{{location}}'</rdfs:comment>
    <rdfs:domain rdf:resource="http://example.org/onto/class/google_data_loss_prevention_inspect_template"/>
    <rdfs:range rdf:resource="http://www.w3.org/2001/XMLSchema#string"/>
  </owl:DatatypeProperty>
  <owl:DatatypeProperty rdf:about="http://example.org/onto/prop/google_data_loss_prevention_inspect_template_template_id">
    <rdfs:label>template_id</rdfs:label>
    <rdfs:comment>The template id can contain uppercase and lowercase letters, numbers, and hyphens;
that is, it must match the regular expression: [a-zA-Z\d-_]+. The maximum length is
100 characters. Can be empty to allow the system to generate one.</rdfs:comment>
    <rdfs:domain rdf:resource="http://example.org/onto/class/google_data_loss_prevention_inspect_template"/>
    <rdfs:range rdf:resource="http://www.w3.org/2001/XMLSchema#string"/>
  </owl:DatatypeProperty>
  <owl:DatatypeProperty rdf:about="http://example.org/onto/prop/google_data_loss_prevention_inspect_template_content_options">
    <rdfs:label>content_options</rdfs:label>
    <rdfs:comment>List of options defining data content to scan. If empty, text, images, and other content will be included. Possible values: ["CONTENT_TEXT", "CONTENT_IMAGE"]</rdfs:comment>
    <rdfs:domain rdf:resource="http://example.org/onto/class/google_data_loss_prevention_inspect_template"/>
    <rdfs:range rdf:resource="http://www.w3.org/2001/XMLSchema#string"/>
  </owl:DatatypeProperty>
  <owl:DatatypeProperty rdf:about="http://example.org/onto/prop/google_data_loss_prevention_inspect_template_exclude_info_types">
    <rdfs:label>exclude_info_types</rdfs:label>
    <rdfs:comment>When true, excludes type information of the findings.</rdfs:comment>
    <rdfs:domain rdf:resource="http://example.org/onto/class/google_data_loss_prevention_inspect_template"/>
    <rdfs:range rdf:resource="http://www.w3.org/2001/XMLSchema#string"/>
  </owl:DatatypeProperty>
  <owl:DatatypeProperty rdf:about="http://example.org/onto/prop/google_data_loss_prevention_inspect_template_include_quote">
    <rdfs:label>include_quote</rdfs:label>
    <rdfs:comment>When true, a contextual quote from the data that triggered a finding is included in the response.</rdfs:comment>
    <rdfs:domain rdf:resource="http://example.org/onto/class/google_data_loss_prevention_inspect_template"/>
    <rdfs:range rdf:resource="http://www.w3.org/2001/XMLSchema#string"/>
  </owl:DatatypeProperty>
  <owl:DatatypeProperty rdf:about="http://example.org/onto/prop/google_data_loss_prevention_inspect_template_min_likelihood">
    <rdfs:label>min_likelihood</rdfs:label>
    <rdfs:comment>Only returns findings equal or above this threshold. See https://cloud.google.com/dlp/docs/likelihood for more info Default value: "POSSIBLE" Possible values: ["VERY_UNLIKELY", "UNLIKELY", "POSSIBLE", "LIKELY", "VERY_LIKELY"]</rdfs:comment>
    <rdfs:domain rdf:resource="http://example.org/onto/class/google_data_loss_prevention_inspect_template"/>
    <rdfs:range rdf:resource="http://www.w3.org/2001/XMLSchema#string"/>
  </owl:DatatypeProperty>
  <owl:DatatypeProperty rdf:about="http://example.org/onto/prop/google_data_loss_prevention_inspect_template_exclusion_type">
    <rdfs:label>exclusion_type</rdfs:label>
    <rdfs:comment>If set to EXCLUSION_TYPE_EXCLUDE this infoType will not cause a finding to be returned. It still can be used for rules matching. Possible values: ["EXCLUSION_TYPE_EXCLUDE"]</rdfs:comment>
    <rdfs:domain rdf:resource="http://example.org/onto/class/google_data_loss_prevention_inspect_template"/>
    <rdfs:range rdf:resource="http://www.w3.org/2001/XMLSchema#string"/>
  </owl:DatatypeProperty>
  <owl:DatatypeProperty rdf:about="http://example.org/onto/prop/google_data_loss_prevention_inspect_template_likelihood">
    <rdfs:label>likelihood</rdfs:label>
    <rdfs:comment>Likelihood to return for this CustomInfoType. This base value can be altered by a detection rule if the finding meets the criteria
specified by the rule. Default value: "VERY_LIKELY" Possible values: ["VERY_UNLIKELY", "UNLIKELY", "POSSIBLE", "LIKELY", "VERY_LIKELY"]</rdfs:comment>
    <rdfs:domain rdf:resource="http://example.org/onto/class/google_data_loss_prevention_inspect_template"/>
    <rdfs:range rdf:resource="http://www.w3.org/2001/XMLSchema#string"/>
  </owl:DatatypeProperty>
  <owl:DatatypeProperty rdf:about="http://example.org/onto/prop/google_data_loss_prevention_inspect_template_path">
    <rdfs:label>path</rdfs:label>
    <rdfs:comment>A url representing a file or path (no wildcards) in Cloud Storage. Example: 'gs://[BUCKET_NAME]/dictionary.txt'</rdfs:comment>
    <rdfs:domain rdf:resource="http://example.org/onto/class/google_data_loss_prevention_inspect_template"/>
    <rdfs:range rdf:resource="http://www.w3.org/2001/XMLSchema#string"/>
  </owl:DatatypeProperty>
  <owl:DatatypeProperty rdf:about="http://example.org/onto/prop/google_data_loss_prevention_inspect_template_words">
    <rdfs:label>words</rdfs:label>
    <rdfs:comment>Words or phrases defining the dictionary. The dictionary must contain at least one
phrase and every phrase must contain at least 2 characters that are letters or digits.</rdfs:comment>
    <rdfs:domain rdf:resource="http://example.org/onto/class/google_data_loss_prevention_inspect_template"/>
    <rdfs:range rdf:resource="http://www.w3.org/2001/XMLSchema#string"/>
  </owl:DatatypeProperty>
  <owl:DatatypeProperty rdf:about="http://example.org/onto/prop/google_data_loss_prevention_inspect_template_name">
    <rdfs:label>name</rdfs:label>
    <rdfs:comment>Name of the information type. Either a name of your choosing when creating a CustomInfoType, or one of the names
listed at https://cloud.google.com/dlp/docs/infotypes-reference when specifying a built-in type.</rdfs:comment>
    <rdfs:domain rdf:resource="http://example.org/onto/class/google_data_loss_prevention_inspect_template"/>
    <rdfs:range rdf:resource="http://www.w3.org/2001/XMLSchema#string"/>
  </owl:DatatypeProperty>
  <owl:DatatypeProperty rdf:about="http://example.org/onto/prop/google_data_loss_prevention_inspect_template_version">
    <rdfs:label>version</rdfs:label>
    <rdfs:comment>Version name for this InfoType.</rdfs:comment>
    <rdfs:domain rdf:resource="http://example.org/onto/class/google_data_loss_prevention_inspect_template"/>
    <rdfs:range rdf:resource="http://www.w3.org/2001/XMLSchema#string"/>
  </owl:DatatypeProperty>
  <owl:DatatypeProperty rdf:about="http://example.org/onto/prop/google_data_loss_prevention_inspect_template_score">
    <rdfs:label>score</rdfs:label>
    <rdfs:comment>The sensitivity score applied to the resource. Possible values: ["SENSITIVITY_LOW", "SENSITIVITY_MODERATE", "SENSITIVITY_HIGH"]</rdfs:comment>
    <rdfs:domain rdf:resource="http://example.org/onto/class/google_data_loss_prevention_inspect_template"/>
    <rdfs:range rdf:resource="http://www.w3.org/2001/XMLSchema#string"/>
  </owl:DatatypeProperty>
  <owl:DatatypeProperty rdf:about="http://example.org/onto/prop/google_data_loss_prevention_inspect_template_group_indexes">
    <rdfs:label>group_indexes</rdfs:label>
    <rdfs:comment>The index of the submatch to extract as findings. When not specified, the entire match is returned. No more than 3 may be included.</rdfs:comment>
    <rdfs:domain rdf:resource="http://example.org/onto/class/google_data_loss_prevention_inspect_template"/>
    <rdfs:range rdf:resource="http://www.w3.org/2001/XMLSchema#string"/>
  </owl:DatatypeProperty>
  <owl:DatatypeProperty rdf:about="http://example.org/onto/prop/google_data_loss_prevention_inspect_template_pattern">
    <rdfs:label>pattern</rdfs:label>
    <rdfs:comment>Pattern defining the regular expression.
Its syntax (https://github.com/google/re2/wiki/Syntax) can be found under the google/re2 repository on GitHub.</rdfs:comment>
    <rdfs:domain rdf:resource="http://example.org/onto/class/google_data_loss_prevention_inspect_template"/>
    <rdfs:range rdf:resource="http://www.w3.org/2001/XMLSchema#string"/>
  </owl:DatatypeProperty>
  <owl:DatatypeProperty rdf:about="http://example.org/onto/prop/google_data_loss_prevention_inspect_template_score">
    <rdfs:label>score</rdfs:label>
    <rdfs:comment>The sensitivity score applied to the resource. Possible values: ["SENSITIVITY_LOW", "SENSITIVITY_MODERATE", "SENSITIVITY_HIGH"]</rdfs:comment>
    <rdfs:domain rdf:resource="http://example.org/onto/class/google_data_loss_prevention_inspect_template"/>
    <rdfs:range rdf:resource="http://www.w3.org/2001/XMLSchema#string"/>
  </owl:DatatypeProperty>
  <owl:DatatypeProperty rdf:about="http://example.org/onto/prop/google_data_loss_prevention_inspect_template_name">
    <rdfs:label>name</rdfs:label>
    <rdfs:comment>Resource name of the requested StoredInfoType, for example 'organizations/433245324/storedInfoTypes/432452342'
or 'projects/project-id/storedInfoTypes/432452342'.</rdfs:comment>
    <rdfs:domain rdf:resource="http://example.org/onto/class/google_data_loss_prevention_inspect_template"/>
    <rdfs:range rdf:resource="http://www.w3.org/2001/XMLSchema#string"/>
  </owl:DatatypeProperty>
  <owl:DatatypeProperty rdf:about="http://example.org/onto/prop/google_data_loss_prevention_inspect_template_name">
    <rdfs:label>name</rdfs:label>
    <rdfs:comment>Name of the information type. Either a name of your choosing when creating a CustomInfoType, or one of the names listed
at https://cloud.google.com/dlp/docs/infotypes-reference when specifying a built-in type.</rdfs:comment>
    <rdfs:domain rdf:resource="http://example.org/onto/class/google_data_loss_prevention_inspect_template"/>
    <rdfs:range rdf:resource="http://www.w3.org/2001/XMLSchema#string"/>
  </owl:DatatypeProperty>
  <owl:DatatypeProperty rdf:about="http://example.org/onto/prop/google_data_loss_prevention_inspect_template_version">
    <rdfs:label>version</rdfs:label>
    <rdfs:comment>Version of the information type to use. By default, the version is set to stable</rdfs:comment>
    <rdfs:domain rdf:resource="http://example.org/onto/class/google_data_loss_prevention_inspect_template"/>
    <rdfs:range rdf:resource="http://www.w3.org/2001/XMLSchema#string"/>
  </owl:DatatypeProperty>
  <owl:DatatypeProperty rdf:about="http://example.org/onto/prop/google_data_loss_prevention_inspect_template_score">
    <rdfs:label>score</rdfs:label>
    <rdfs:comment>The sensitivity score applied to the resource. Possible values: ["SENSITIVITY_LOW", "SENSITIVITY_MODERATE", "SENSITIVITY_HIGH"]</rdfs:comment>
    <rdfs:domain rdf:resource="http://example.org/onto/class/google_data_loss_prevention_inspect_template"/>
    <rdfs:range rdf:resource="http://www.w3.org/2001/XMLSchema#string"/>
  </owl:DatatypeProperty>
  <owl:DatatypeProperty rdf:about="http://example.org/onto/prop/google_data_loss_prevention_inspect_template_max_findings_per_item">
    <rdfs:label>max_findings_per_item</rdfs:label>
    <rdfs:comment>Max number of findings that will be returned for each item scanned. The maximum returned is 2000.</rdfs:comment>
    <rdfs:domain rdf:resource="http://example.org/onto/class/google_data_loss_prevention_inspect_template"/>
    <rdfs:range rdf:resource="http://www.w3.org/2001/XMLSchema#string"/>
  </owl:DatatypeProperty>
  <owl:DatatypeProperty rdf:about="http://example.org/onto/prop/google_data_loss_prevention_inspect_template_max_findings_per_request">
    <rdfs:label>max_findings_per_request</rdfs:label>
    <rdfs:comment>Max number of findings that will be returned per request/job. The maximum returned is 2000.</rdfs:comment>
    <rdfs:domain rdf:resource="http://example.org/onto/class/google_data_loss_prevention_inspect_template"/>
    <rdfs:range rdf:resource="http://www.w3.org/2001/XMLSchema#string"/>
  </owl:DatatypeProperty>
  <owl:DatatypeProperty rdf:about="http://example.org/onto/prop/google_data_loss_prevention_inspect_template_max_findings">
    <rdfs:label>max_findings</rdfs:label>
    <rdfs:comment>Max findings limit for the given infoType.</rdfs:comment>
    <rdfs:domain rdf:resource="http://example.org/onto/class/google_data_loss_prevention_inspect_template"/>
    <rdfs:range rdf:resource="http://www.w3.org/2001/XMLSchema#string"/>
  </owl:DatatypeProperty>
  <owl:DatatypeProperty rdf:about="http://example.org/onto/prop/google_data_loss_prevention_inspect_template_name">
    <rdfs:label>name</rdfs:label>
    <rdfs:comment>Name of the information type. Either a name of your choosing when creating a CustomInfoType, or one of the names listed
at https://cloud.google.com/dlp/docs/infotypes-reference when specifying a built-in type.</rdfs:comment>
    <rdfs:domain rdf:resource="http://example.org/onto/class/google_data_loss_prevention_inspect_template"/>
    <rdfs:range rdf:resource="http://www.w3.org/2001/XMLSchema#string"/>
  </owl:DatatypeProperty>
  <owl:DatatypeProperty rdf:about="http://example.org/onto/prop/google_data_loss_prevention_inspect_template_version">
    <rdfs:label>version</rdfs:label>
    <rdfs:comment>Version name for this InfoType.</rdfs:comment>
    <rdfs:domain rdf:resource="http://example.org/onto/class/google_data_loss_prevention_inspect_template"/>
    <rdfs:range rdf:resource="http://www.w3.org/2001/XMLSchema#string"/>
  </owl:DatatypeProperty>
  <owl:DatatypeProperty rdf:about="http://example.org/onto/prop/google_data_loss_prevention_inspect_template_score">
    <rdfs:label>score</rdfs:label>
    <rdfs:comment>The sensitivity score applied to the resource. Possible values: ["SENSITIVITY_LOW", "SENSITIVITY_MODERATE", "SENSITIVITY_HIGH"]</rdfs:comment>
    <rdfs:domain rdf:resource="http://example.org/onto/class/google_data_loss_prevention_inspect_template"/>
    <rdfs:range rdf:resource="http://www.w3.org/2001/XMLSchema#string"/>
  </owl:DatatypeProperty>
  <owl:DatatypeProperty rdf:about="http://example.org/onto/prop/google_data_loss_prevention_inspect_template_name">
    <rdfs:label>name</rdfs:label>
    <rdfs:comment>Name of the information type. Either a name of your choosing when creating a CustomInfoType, or one of the names listed
at https://cloud.google.com/dlp/docs/infotypes-reference when specifying a built-in type.</rdfs:comment>
    <rdfs:domain rdf:resource="http://example.org/onto/class/google_data_loss_prevention_inspect_template"/>
    <rdfs:range rdf:resource="http://www.w3.org/2001/XMLSchema#string"/>
  </owl:DatatypeProperty>
  <owl:DatatypeProperty rdf:about="http://example.org/onto/prop/google_data_loss_prevention_inspect_template_version">
    <rdfs:label>version</rdfs:label>
    <rdfs:comment>Version name for this InfoType.</rdfs:comment>
    <rdfs:domain rdf:resource="http://example.org/onto/class/google_data_loss_prevention_inspect_template"/>
    <rdfs:range rdf:resource="http://www.w3.org/2001/XMLSchema#string"/>
  </owl:DatatypeProperty>
  <owl:DatatypeProperty rdf:about="http://example.org/onto/prop/google_data_loss_prevention_inspect_template_score">
    <rdfs:label>score</rdfs:label>
    <rdfs:comment>The sensitivity score applied to the resource. Possible values: ["SENSITIVITY_LOW", "SENSITIVITY_MODERATE", "SENSITIVITY_HIGH"]</rdfs:comment>
    <rdfs:domain rdf:resource="http://example.org/onto/class/google_data_loss_prevention_inspect_template"/>
    <rdfs:range rdf:resource="http://www.w3.org/2001/XMLSchema#string"/>
  </owl:DatatypeProperty>
  <owl:DatatypeProperty rdf:about="http://example.org/onto/prop/google_data_loss_prevention_inspect_template_matching_type">
    <rdfs:label>matching_type</rdfs:label>
    <rdfs:comment>How the rule is applied. See the documentation for more information: https://cloud.google.com/dlp/docs/reference/rest/v2/InspectConfig#MatchingType Possible values: ["MATCHING_TYPE_FULL_MATCH", "MATCHING_TYPE_PARTIAL_MATCH", "MATCHING_TYPE_INVERSE_MATCH"]</rdfs:comment>
    <rdfs:domain rdf:resource="http://example.org/onto/class/google_data_loss_prevention_inspect_template"/>
    <rdfs:range rdf:resource="http://www.w3.org/2001/XMLSchema#string"/>
  </owl:DatatypeProperty>
  <owl:DatatypeProperty rdf:about="http://example.org/onto/prop/google_data_loss_prevention_inspect_template_path">
    <rdfs:label>path</rdfs:label>
    <rdfs:comment>A url representing a file or path (no wildcards) in Cloud Storage. Example: 'gs://[BUCKET_NAME]/dictionary.txt'</rdfs:comment>
    <rdfs:domain rdf:resource="http://example.org/onto/class/google_data_loss_prevention_inspect_template"/>
    <rdfs:range rdf:resource="http://www.w3.org/2001/XMLSchema#string"/>
  </owl:DatatypeProperty>
  <owl:DatatypeProperty rdf:about="http://example.org/onto/prop/google_data_loss_prevention_inspect_template_words">
    <rdfs:label>words</rdfs:label>
    <rdfs:comment>Words or phrases defining the dictionary. The dictionary must contain at least one
phrase and every phrase must contain at least 2 characters that are letters or digits.</rdfs:comment>
    <rdfs:domain rdf:resource="http://example.org/onto/class/google_data_loss_prevention_inspect_template"/>
    <rdfs:range rdf:resource="http://www.w3.org/2001/XMLSchema#string"/>
  </owl:DatatypeProperty>
  <owl:DatatypeProperty rdf:about="http://example.org/onto/prop/google_data_loss_prevention_inspect_template_group_indexes">
    <rdfs:label>group_indexes</rdfs:label>
    <rdfs:comment>The index of the submatch to extract as findings. When not specified,
the entire match is returned. No more than 3 may be included.</rdfs:comment>
    <rdfs:domain rdf:resource="http://example.org/onto/class/google_data_loss_prevention_inspect_template"/>
    <rdfs:range rdf:resource="http://www.w3.org/2001/XMLSchema#string"/>
  </owl:DatatypeProperty>
  <owl:DatatypeProperty rdf:about="http://example.org/onto/prop/google_data_loss_prevention_inspect_template_pattern">
    <rdfs:label>pattern</rdfs:label>
    <rdfs:comment>Pattern defining the regular expression. Its syntax
(https://github.com/google/re2/wiki/Syntax) can be found under the google/re2 repository on GitHub.</rdfs:comment>
    <rdfs:domain rdf:resource="http://example.org/onto/class/google_data_loss_prevention_inspect_template"/>
    <rdfs:range rdf:resource="http://www.w3.org/2001/XMLSchema#string"/>
  </owl:DatatypeProperty>
  <owl:DatatypeProperty rdf:about="http://example.org/onto/prop/google_data_loss_prevention_inspect_template_window_after">
    <rdfs:label>window_after</rdfs:label>
    <rdfs:comment>Number of characters after the finding to consider.</rdfs:comment>
    <rdfs:domain rdf:resource="http://example.org/onto/class/google_data_loss_prevention_inspect_template"/>
    <rdfs:range rdf:resource="http://www.w3.org/2001/XMLSchema#string"/>
  </owl:DatatypeProperty>
  <owl:DatatypeProperty rdf:about="http://example.org/onto/prop/google_data_loss_prevention_inspect_template_window_before">
    <rdfs:label>window_before</rdfs:label>
    <rdfs:comment>Number of characters before the finding to consider.</rdfs:comment>
    <rdfs:domain rdf:resource="http://example.org/onto/class/google_data_loss_prevention_inspect_template"/>
    <rdfs:range rdf:resource="http://www.w3.org/2001/XMLSchema#string"/>
  </owl:DatatypeProperty>
  <owl:DatatypeProperty rdf:about="http://example.org/onto/prop/google_data_loss_prevention_inspect_template_name">
    <rdfs:label>name</rdfs:label>
    <rdfs:comment>Name of the information type. Either a name of your choosing when creating a CustomInfoType, or one of the names listed
at https://cloud.google.com/dlp/docs/infotypes-reference when specifying a built-in type.</rdfs:comment>
    <rdfs:domain rdf:resource="http://example.org/onto/class/google_data_loss_prevention_inspect_template"/>
    <rdfs:range rdf:resource="http://www.w3.org/2001/XMLSchema#string"/>
  </owl:DatatypeProperty>
  <owl:DatatypeProperty rdf:about="http://example.org/onto/prop/google_data_loss_prevention_inspect_template_version">
    <rdfs:label>version</rdfs:label>
    <rdfs:comment>Version name for this InfoType.</rdfs:comment>
    <rdfs:domain rdf:resource="http://example.org/onto/class/google_data_loss_prevention_inspect_template"/>
    <rdfs:range rdf:resource="http://www.w3.org/2001/XMLSchema#string"/>
  </owl:DatatypeProperty>
  <owl:DatatypeProperty rdf:about="http://example.org/onto/prop/google_data_loss_prevention_inspect_template_score">
    <rdfs:label>score</rdfs:label>
    <rdfs:comment>The sensitivity score applied to the resource. Possible values: ["SENSITIVITY_LOW", "SENSITIVITY_MODERATE", "SENSITIVITY_HIGH"]</rdfs:comment>
    <rdfs:domain rdf:resource="http://example.org/onto/class/google_data_loss_prevention_inspect_template"/>
    <rdfs:range rdf:resource="http://www.w3.org/2001/XMLSchema#string"/>
  </owl:DatatypeProperty>
  <owl:DatatypeProperty rdf:about="http://example.org/onto/prop/google_data_loss_prevention_inspect_template_group_indexes">
    <rdfs:label>group_indexes</rdfs:label>
    <rdfs:comment>The index of the submatch to extract as findings. When not specified, the entire match is returned. No more than 3 may be included.</rdfs:comment>
    <rdfs:domain rdf:resource="http://example.org/onto/class/google_data_loss_prevention_inspect_template"/>
    <rdfs:range rdf:resource="http://www.w3.org/2001/XMLSchema#string"/>
  </owl:DatatypeProperty>
  <owl:DatatypeProperty rdf:about="http://example.org/onto/prop/google_data_loss_prevention_inspect_template_pattern">
    <rdfs:label>pattern</rdfs:label>
    <rdfs:comment>Pattern defining the regular expression.
Its syntax (https://github.com/google/re2/wiki/Syntax) can be found under the google/re2 repository on GitHub.</rdfs:comment>
    <rdfs:domain rdf:resource="http://example.org/onto/class/google_data_loss_prevention_inspect_template"/>
    <rdfs:range rdf:resource="http://www.w3.org/2001/XMLSchema#string"/>
  </owl:DatatypeProperty>
  <owl:DatatypeProperty rdf:about="http://example.org/onto/prop/google_data_loss_prevention_inspect_template_group_indexes">
    <rdfs:label>group_indexes</rdfs:label>
    <rdfs:comment>The index of the submatch to extract as findings. When not specified,
the entire match is returned. No more than 3 may be included.</rdfs:comment>
    <rdfs:domain rdf:resource="http://example.org/onto/class/google_data_loss_prevention_inspect_template"/>
    <rdfs:range rdf:resource="http://www.w3.org/2001/XMLSchema#string"/>
  </owl:DatatypeProperty>
  <owl:DatatypeProperty rdf:about="http://example.org/onto/prop/google_data_loss_prevention_inspect_template_pattern">
    <rdfs:label>pattern</rdfs:label>
    <rdfs:comment>Pattern defining the regular expression. Its syntax
(https://github.com/google/re2/wiki/Syntax) can be found under the google/re2 repository on GitHub.</rdfs:comment>
    <rdfs:domain rdf:resource="http://example.org/onto/class/google_data_loss_prevention_inspect_template"/>
    <rdfs:range rdf:resource="http://www.w3.org/2001/XMLSchema#string"/>
  </owl:DatatypeProperty>
  <owl:DatatypeProperty rdf:about="http://example.org/onto/prop/google_data_loss_prevention_inspect_template_fixed_likelihood">
    <rdfs:label>fixed_likelihood</rdfs:label>
    <rdfs:comment>Set the likelihood of a finding to a fixed value. Either this or relative_likelihood can be set. Possible values: ["VERY_UNLIKELY", "UNLIKELY", "POSSIBLE", "LIKELY", "VERY_LIKELY"]</rdfs:comment>
    <rdfs:domain rdf:resource="http://example.org/onto/class/google_data_loss_prevention_inspect_template"/>
    <rdfs:range rdf:resource="http://www.w3.org/2001/XMLSchema#string"/>
  </owl:DatatypeProperty>
  <owl:DatatypeProperty rdf:about="http://example.org/onto/prop/google_data_loss_prevention_inspect_template_relative_likelihood">
    <rdfs:label>relative_likelihood</rdfs:label>
    <rdfs:comment>Increase or decrease the likelihood by the specified number of levels. For example,
if a finding would be POSSIBLE without the detection rule and relativeLikelihood is 1,
then it is upgraded to LIKELY, while a value of -1 would downgrade it to UNLIKELY.
Likelihood may never drop below VERY_UNLIKELY or exceed VERY_LIKELY, so applying an
adjustment of 1 followed by an adjustment of -1 when base likelihood is VERY_LIKELY
will result in a final likelihood of LIKELY. Either this or fixed_likelihood can be set.</rdfs:comment>
    <rdfs:domain rdf:resource="http://example.org/onto/class/google_data_loss_prevention_inspect_template"/>
    <rdfs:range rdf:resource="http://www.w3.org/2001/XMLSchema#string"/>
  </owl:DatatypeProperty>
  <owl:DatatypeProperty rdf:about="http://example.org/onto/prop/google_data_loss_prevention_inspect_template_window_after">
    <rdfs:label>window_after</rdfs:label>
    <rdfs:comment>Number of characters after the finding to consider. Either this or window_before must be specified</rdfs:comment>
    <rdfs:domain rdf:resource="http://example.org/onto/class/google_data_loss_prevention_inspect_template"/>
    <rdfs:range rdf:resource="http://www.w3.org/2001/XMLSchema#string"/>
  </owl:DatatypeProperty>
  <owl:DatatypeProperty rdf:about="http://example.org/onto/prop/google_data_loss_prevention_inspect_template_window_before">
    <rdfs:label>window_before</rdfs:label>
    <rdfs:comment>Number of characters before the finding to consider. Either this or window_after must be specified</rdfs:comment>
    <rdfs:domain rdf:resource="http://example.org/onto/class/google_data_loss_prevention_inspect_template"/>
    <rdfs:range rdf:resource="http://www.w3.org/2001/XMLSchema#string"/>
  </owl:DatatypeProperty>
  <owl:DatatypeProperty rdf:about="http://example.org/onto/prop/google_data_loss_prevention_inspect_template_create">
    <rdfs:label>create</rdfs:label>
    <rdfs:domain rdf:resource="http://example.org/onto/class/google_data_loss_prevention_inspect_template"/>
    <rdfs:range rdf:resource="http://www.w3.org/2001/XMLSchema#string"/>
  </owl:DatatypeProperty>
  <owl:DatatypeProperty rdf:about="http://example.org/onto/prop/google_data_loss_prevention_inspect_template_delete">
    <rdfs:label>delete</rdfs:label>
    <rdfs:domain rdf:resource="http://example.org/onto/class/google_data_loss_prevention_inspect_template"/>
    <rdfs:range rdf:resource="http://www.w3.org/2001/XMLSchema#string"/>
  </owl:DatatypeProperty>
  <owl:DatatypeProperty rdf:about="http://example.org/onto/prop/google_data_loss_prevention_inspect_template_update">
    <rdfs:label>update</rdfs:label>
    <rdfs:domain rdf:resource="http://example.org/onto/class/google_data_loss_prevention_inspect_template"/>
    <rdfs:range rdf:resource="http://www.w3.org/2001/XMLSchema#string"/>
  </owl:DatatypeProperty>
</rdf:RDF>
