<?xml version="1.0" encoding="UTF-8"?>
<rdf:RDF
  xmlns:rdf="http://www.w3.org/1999/02/22-rdf-syntax-ns#"
  xmlns:rdfs="http://www.w3.org/2000/01/rdf-schema#"
  xmlns:owl="http://www.w3.org/2002/07/owl#"
  xmlns:xsd="http://www.w3.org/2001/XMLSchema#"
  xml:base="http://example.org/onto/">
  <owl:Class rdf:about="http://example.org/onto/class/google_netapp_backup">
    <rdfs:label>google_netapp_backup</rdfs:label>
    <rdfs:comment>#
#     ***     AUTO GENERATED CODE    ***    Type: MMv1     ***
#
# ----------------------------------------------------------------------------
#
#     This code is generated by Magic Modules using the following:
#
#     Configuration: https:#github.com/GoogleCloudPlatform/magic-modules/tree/main/mmv1/products/netapp/Backup.yaml
#     Template:      https:#github.com/GoogleCloudPlatform/magic-modules/tree/main/mmv1/templates/terraform/resource.html.markdown.tmpl
#
#     DO NOT EDIT this file directly. Any changes made to this file will be
#     overwritten during the next generation cycle.
#
# ----------------------------------------------------------------------------
subcategory: "Google Cloud NetApp Volumes"
description: |-
  NetApp Volumes supports volume backups, which are copies of your volumes
  stored independently from the volume.
---</rdfs:comment>
  </owl:Class>
  <owl:DatatypeProperty rdf:about="http://example.org/onto/prop/google_netapp_backup_backup_region">
    <rdfs:label>backup_region</rdfs:label>
    <rdfs:comment>Region in which backup is stored.</rdfs:comment>
    <rdfs:domain rdf:resource="http://example.org/onto/class/google_netapp_backup"/>
    <rdfs:range rdf:resource="http://www.w3.org/2001/XMLSchema#string"/>
  </owl:DatatypeProperty>
  <owl:DatatypeProperty rdf:about="http://example.org/onto/prop/google_netapp_backup_backup_type">
    <rdfs:label>backup_type</rdfs:label>
    <rdfs:comment>Type of backup, manually created or created by a backup policy. Possible Values : [TYPE_UNSPECIFIED, MANUAL, SCHEDULED]</rdfs:comment>
    <rdfs:domain rdf:resource="http://example.org/onto/class/google_netapp_backup"/>
    <rdfs:range rdf:resource="http://www.w3.org/2001/XMLSchema#string"/>
  </owl:DatatypeProperty>
  <owl:DatatypeProperty rdf:about="http://example.org/onto/prop/google_netapp_backup_chain_storage_bytes">
    <rdfs:label>chain_storage_bytes</rdfs:label>
    <rdfs:comment>Backups of a volume build incrementally on top of each other. They form a "backup chain".
Total size of all backups in a chain in bytes = baseline backup size + sum(incremental backup size)</rdfs:comment>
    <rdfs:domain rdf:resource="http://example.org/onto/class/google_netapp_backup"/>
    <rdfs:range rdf:resource="http://www.w3.org/2001/XMLSchema#string"/>
  </owl:DatatypeProperty>
  <owl:DatatypeProperty rdf:about="http://example.org/onto/prop/google_netapp_backup_create_time">
    <rdfs:label>create_time</rdfs:label>
    <rdfs:comment>Create time of the backup. A timestamp in RFC3339 UTC "Zulu" format. Examples: "2023-06-22T09:13:01.617Z".</rdfs:comment>
    <rdfs:domain rdf:resource="http://example.org/onto/class/google_netapp_backup"/>
    <rdfs:range rdf:resource="http://www.w3.org/2001/XMLSchema#string"/>
  </owl:DatatypeProperty>
  <owl:DatatypeProperty rdf:about="http://example.org/onto/prop/google_netapp_backup_description">
    <rdfs:label>description</rdfs:label>
    <rdfs:comment>A description of the backup with 2048 characters or less. Requests with longer descriptions will be rejected.</rdfs:comment>
    <rdfs:domain rdf:resource="http://example.org/onto/class/google_netapp_backup"/>
    <rdfs:range rdf:resource="http://www.w3.org/2001/XMLSchema#string"/>
  </owl:DatatypeProperty>
  <owl:DatatypeProperty rdf:about="http://example.org/onto/prop/google_netapp_backup_effective_labels">
    <rdfs:label>effective_labels</rdfs:label>
    <rdfs:comment>All of labels (key/value pairs) present on the resource in GCP, including the labels configured through Terraform, other clients and services.</rdfs:comment>
    <rdfs:domain rdf:resource="http://example.org/onto/class/google_netapp_backup"/>
    <rdfs:range rdf:resource="http://www.w3.org/2001/XMLSchema#string"/>
  </owl:DatatypeProperty>
  <owl:DatatypeProperty rdf:about="http://example.org/onto/prop/google_netapp_backup_id">
    <rdfs:label>id</rdfs:label>
    <rdfs:domain rdf:resource="http://example.org/onto/class/google_netapp_backup"/>
    <rdfs:range rdf:resource="http://www.w3.org/2001/XMLSchema#string"/>
  </owl:DatatypeProperty>
  <owl:DatatypeProperty rdf:about="http://example.org/onto/prop/google_netapp_backup_labels">
    <rdfs:label>labels</rdfs:label>
    <rdfs:comment>Labels as key value pairs. Example: '{ "owner": "Bob", "department": "finance", "purpose": "testing" }'.


**Note**: This field is non-authoritative, and will only manage the labels present in your configuration.
Please refer to the field 'effective_labels' for all of the labels present on the resource.</rdfs:comment>
    <rdfs:domain rdf:resource="http://example.org/onto/class/google_netapp_backup"/>
    <rdfs:range rdf:resource="http://www.w3.org/2001/XMLSchema#string"/>
  </owl:DatatypeProperty>
  <owl:DatatypeProperty rdf:about="http://example.org/onto/prop/google_netapp_backup_location">
    <rdfs:label>location</rdfs:label>
    <rdfs:comment>Location of the backup.</rdfs:comment>
    <rdfs:domain rdf:resource="http://example.org/onto/class/google_netapp_backup"/>
    <rdfs:range rdf:resource="http://www.w3.org/2001/XMLSchema#string"/>
  </owl:DatatypeProperty>
  <owl:DatatypeProperty rdf:about="http://example.org/onto/prop/google_netapp_backup_name">
    <rdfs:label>name</rdfs:label>
    <rdfs:comment>The resource name of the backup. Needs to be unique per location.</rdfs:comment>
    <rdfs:domain rdf:resource="http://example.org/onto/class/google_netapp_backup"/>
    <rdfs:range rdf:resource="http://www.w3.org/2001/XMLSchema#string"/>
  </owl:DatatypeProperty>
  <owl:DatatypeProperty rdf:about="http://example.org/onto/prop/google_netapp_backup_project">
    <rdfs:label>project</rdfs:label>
    <rdfs:domain rdf:resource="http://example.org/onto/class/google_netapp_backup"/>
    <rdfs:range rdf:resource="http://www.w3.org/2001/XMLSchema#string"/>
  </owl:DatatypeProperty>
  <owl:DatatypeProperty rdf:about="http://example.org/onto/prop/google_netapp_backup_source_snapshot">
    <rdfs:label>source_snapshot</rdfs:label>
    <rdfs:comment>If specified, backup will be created from the given snapshot. If not specified,
there will be a new snapshot taken to initiate the backup creation.
Format: 'projects/{{projectId}}/locations/{{location}}/volumes/{{volumename}}/snapshots/{{snapshotname}}''</rdfs:comment>
    <rdfs:domain rdf:resource="http://example.org/onto/class/google_netapp_backup"/>
    <rdfs:range rdf:resource="http://www.w3.org/2001/XMLSchema#string"/>
  </owl:DatatypeProperty>
  <owl:DatatypeProperty rdf:about="http://example.org/onto/prop/google_netapp_backup_source_volume">
    <rdfs:label>source_volume</rdfs:label>
    <rdfs:comment>ID of volumes this backup belongs to. Format: 'projects/{{projects_id}}/locations/{{location}}/volumes/{{name}}''</rdfs:comment>
    <rdfs:domain rdf:resource="http://example.org/onto/class/google_netapp_backup"/>
    <rdfs:range rdf:resource="http://www.w3.org/2001/XMLSchema#string"/>
  </owl:DatatypeProperty>
  <owl:DatatypeProperty rdf:about="http://example.org/onto/prop/google_netapp_backup_state">
    <rdfs:label>state</rdfs:label>
    <rdfs:comment>The state of the Backup Vault. Possible Values : [STATE_UNSPECIFIED, CREATING, UPLOADING, READY, DELETING, ERROR, UPDATING]</rdfs:comment>
    <rdfs:domain rdf:resource="http://example.org/onto/class/google_netapp_backup"/>
    <rdfs:range rdf:resource="http://www.w3.org/2001/XMLSchema#string"/>
  </owl:DatatypeProperty>
  <owl:DatatypeProperty rdf:about="http://example.org/onto/prop/google_netapp_backup_terraform_labels">
    <rdfs:label>terraform_labels</rdfs:label>
    <rdfs:comment>The combination of labels configured directly on the resource
 and default labels configured on the provider.</rdfs:comment>
    <rdfs:domain rdf:resource="http://example.org/onto/class/google_netapp_backup"/>
    <rdfs:range rdf:resource="http://www.w3.org/2001/XMLSchema#string"/>
  </owl:DatatypeProperty>
  <owl:DatatypeProperty rdf:about="http://example.org/onto/prop/google_netapp_backup_vault_name">
    <rdfs:label>vault_name</rdfs:label>
    <rdfs:comment>Name of the backup vault to store the backup in.</rdfs:comment>
    <rdfs:domain rdf:resource="http://example.org/onto/class/google_netapp_backup"/>
    <rdfs:range rdf:resource="http://www.w3.org/2001/XMLSchema#string"/>
  </owl:DatatypeProperty>
  <owl:DatatypeProperty rdf:about="http://example.org/onto/prop/google_netapp_backup_volume_region">
    <rdfs:label>volume_region</rdfs:label>
    <rdfs:comment>Region of the volume from which the backup was created.</rdfs:comment>
    <rdfs:domain rdf:resource="http://example.org/onto/class/google_netapp_backup"/>
    <rdfs:range rdf:resource="http://www.w3.org/2001/XMLSchema#string"/>
  </owl:DatatypeProperty>
  <owl:DatatypeProperty rdf:about="http://example.org/onto/prop/google_netapp_backup_volume_usage_bytes">
    <rdfs:label>volume_usage_bytes</rdfs:label>
    <rdfs:comment>Size of the file system when the backup was created. When creating a new volume from the backup, the volume capacity will have to be at least as big.</rdfs:comment>
    <rdfs:domain rdf:resource="http://example.org/onto/class/google_netapp_backup"/>
    <rdfs:range rdf:resource="http://www.w3.org/2001/XMLSchema#string"/>
  </owl:DatatypeProperty>
  <owl:DatatypeProperty rdf:about="http://example.org/onto/prop/google_netapp_backup_create">
    <rdfs:label>create</rdfs:label>
    <rdfs:domain rdf:resource="http://example.org/onto/class/google_netapp_backup"/>
    <rdfs:range rdf:resource="http://www.w3.org/2001/XMLSchema#string"/>
  </owl:DatatypeProperty>
  <owl:DatatypeProperty rdf:about="http://example.org/onto/prop/google_netapp_backup_delete">
    <rdfs:label>delete</rdfs:label>
    <rdfs:domain rdf:resource="http://example.org/onto/class/google_netapp_backup"/>
    <rdfs:range rdf:resource="http://www.w3.org/2001/XMLSchema#string"/>
  </owl:DatatypeProperty>
  <owl:DatatypeProperty rdf:about="http://example.org/onto/prop/google_netapp_backup_update">
    <rdfs:label>update</rdfs:label>
    <rdfs:domain rdf:resource="http://example.org/onto/class/google_netapp_backup"/>
    <rdfs:range rdf:resource="http://www.w3.org/2001/XMLSchema#string"/>
  </owl:DatatypeProperty>
</rdf:RDF>
