<?xml version="1.0" encoding="UTF-8"?>
<rdf:RDF
  xmlns:rdf="http://www.w3.org/1999/02/22-rdf-syntax-ns#"
  xmlns:rdfs="http://www.w3.org/2000/01/rdf-schema#"
  xmlns:owl="http://www.w3.org/2002/07/owl#"
  xmlns:xsd="http://www.w3.org/2001/XMLSchema#"
  xml:base="http://example.org/onto/">
  <owl:Class rdf:about="http://example.org/onto/class/google_spanner_database">
    <rdfs:label>google_spanner_database</rdfs:label>
    <rdfs:comment>#
#     ***     AUTO GENERATED CODE    ***    Type: MMv1     ***
#
# ----------------------------------------------------------------------------
#
#     This code is generated by Magic Modules using the following:
#
#     Configuration: https:#github.com/GoogleCloudPlatform/magic-modules/tree/main/mmv1/products/spanner/Database.yaml
#     Template:      https:#github.com/GoogleCloudPlatform/magic-modules/tree/main/mmv1/templates/terraform/resource.html.markdown.tmpl
#
#     DO NOT EDIT this file directly. Any changes made to this file will be
#     overwritten during the next generation cycle.
#
# ----------------------------------------------------------------------------
subcategory: "Cloud Spanner"
description: |-
  A Cloud Spanner Database which is hosted on a Spanner instance.
---</rdfs:comment>
  </owl:Class>
  <owl:DatatypeProperty rdf:about="http://example.org/onto/prop/google_spanner_database_database_dialect">
    <rdfs:label>database_dialect</rdfs:label>
    <rdfs:comment>The dialect of the Cloud Spanner Database.
If it is not provided, "GOOGLE_STANDARD_SQL" will be used. Possible values: ["GOOGLE_STANDARD_SQL", "POSTGRESQL"]</rdfs:comment>
    <rdfs:domain rdf:resource="http://example.org/onto/class/google_spanner_database"/>
    <rdfs:range rdf:resource="http://www.w3.org/2001/XMLSchema#string"/>
  </owl:DatatypeProperty>
  <owl:DatatypeProperty rdf:about="http://example.org/onto/prop/google_spanner_database_ddl">
    <rdfs:label>ddl</rdfs:label>
    <rdfs:comment>An optional list of DDL statements to run inside the database. Statements can create
tables, indexes, etc.

During creation these statements execute atomically with the creation of the database
and if there is an error in any statement, the database is not created.

Terraform does not perform drift detection on this field and assumes that the values
recorded in state are accurate. Limited updates to this field are supported, and
newly appended DDL statements can be executed in an update. However, modifications
to prior statements will create a plan that marks the resource for recreation.</rdfs:comment>
    <rdfs:domain rdf:resource="http://example.org/onto/class/google_spanner_database"/>
    <rdfs:range rdf:resource="http://www.w3.org/2001/XMLSchema#string"/>
  </owl:DatatypeProperty>
  <owl:DatatypeProperty rdf:about="http://example.org/onto/prop/google_spanner_database_default_time_zone">
    <rdfs:label>default_time_zone</rdfs:label>
    <rdfs:comment>The default time zone for the database. The default time zone must be a valid name
from the tz database. Default value is "America/Los_angeles".</rdfs:comment>
    <rdfs:domain rdf:resource="http://example.org/onto/class/google_spanner_database"/>
    <rdfs:range rdf:resource="http://www.w3.org/2001/XMLSchema#string"/>
  </owl:DatatypeProperty>
  <owl:DatatypeProperty rdf:about="http://example.org/onto/prop/google_spanner_database_deletion_protection">
    <rdfs:label>deletion_protection</rdfs:label>
    <rdfs:comment>Whether Terraform will be prevented from destroying the database. Defaults to true.
When a'terraform destroy' or 'terraform apply' would delete the database,
the command will fail if this field is not set to false in Terraform state.
When the field is set to true or unset in Terraform state, a 'terraform apply'
or 'terraform destroy' that would delete the database will fail.
When the field is set to false, deleting the database is allowed.</rdfs:comment>
    <rdfs:domain rdf:resource="http://example.org/onto/class/google_spanner_database"/>
    <rdfs:range rdf:resource="http://www.w3.org/2001/XMLSchema#string"/>
  </owl:DatatypeProperty>
  <owl:DatatypeProperty rdf:about="http://example.org/onto/prop/google_spanner_database_enable_drop_protection">
    <rdfs:label>enable_drop_protection</rdfs:label>
    <rdfs:comment>Whether drop protection is enabled for this database. Defaults to false.
Drop protection is different from
the "deletion_protection" attribute in the following ways:
(1) "deletion_protection" only protects the database from deletions in Terraform.
whereas setting “enableDropProtection” to true protects the database from deletions in all interfaces.
(2) Setting "enableDropProtection" to true also prevents the deletion of the parent instance containing the database.
"deletion_protection" attribute does not provide protection against the deletion of the parent instance.</rdfs:comment>
    <rdfs:domain rdf:resource="http://example.org/onto/class/google_spanner_database"/>
    <rdfs:range rdf:resource="http://www.w3.org/2001/XMLSchema#string"/>
  </owl:DatatypeProperty>
  <owl:DatatypeProperty rdf:about="http://example.org/onto/prop/google_spanner_database_id">
    <rdfs:label>id</rdfs:label>
    <rdfs:domain rdf:resource="http://example.org/onto/class/google_spanner_database"/>
    <rdfs:range rdf:resource="http://www.w3.org/2001/XMLSchema#string"/>
  </owl:DatatypeProperty>
  <owl:DatatypeProperty rdf:about="http://example.org/onto/prop/google_spanner_database_instance">
    <rdfs:label>instance</rdfs:label>
    <rdfs:comment>The instance to create the database on.</rdfs:comment>
    <rdfs:domain rdf:resource="http://example.org/onto/class/google_spanner_database"/>
    <rdfs:range rdf:resource="http://www.w3.org/2001/XMLSchema#string"/>
  </owl:DatatypeProperty>
  <owl:DatatypeProperty rdf:about="http://example.org/onto/prop/google_spanner_database_name">
    <rdfs:label>name</rdfs:label>
    <rdfs:comment>A unique identifier for the database, which cannot be changed after the
instance is created. Values are of the form '[a-z][-_a-z0-9]*[a-z0-9]'.</rdfs:comment>
    <rdfs:domain rdf:resource="http://example.org/onto/class/google_spanner_database"/>
    <rdfs:range rdf:resource="http://www.w3.org/2001/XMLSchema#string"/>
  </owl:DatatypeProperty>
  <owl:DatatypeProperty rdf:about="http://example.org/onto/prop/google_spanner_database_project">
    <rdfs:label>project</rdfs:label>
    <rdfs:domain rdf:resource="http://example.org/onto/class/google_spanner_database"/>
    <rdfs:range rdf:resource="http://www.w3.org/2001/XMLSchema#string"/>
  </owl:DatatypeProperty>
  <owl:DatatypeProperty rdf:about="http://example.org/onto/prop/google_spanner_database_state">
    <rdfs:label>state</rdfs:label>
    <rdfs:comment>An explanation of the status of the database.</rdfs:comment>
    <rdfs:domain rdf:resource="http://example.org/onto/class/google_spanner_database"/>
    <rdfs:range rdf:resource="http://www.w3.org/2001/XMLSchema#string"/>
  </owl:DatatypeProperty>
  <owl:DatatypeProperty rdf:about="http://example.org/onto/prop/google_spanner_database_version_retention_period">
    <rdfs:label>version_retention_period</rdfs:label>
    <rdfs:comment>The retention period for the database. The retention period must be between 1 hour
and 7 days, and can be specified in days, hours, minutes, or seconds. For example,
the values 1d, 24h, 1440m, and 86400s are equivalent. Default value is 1h.
If this property is used, you must avoid adding new DDL statements to 'ddl' that
update the database's version_retention_period.</rdfs:comment>
    <rdfs:domain rdf:resource="http://example.org/onto/class/google_spanner_database"/>
    <rdfs:range rdf:resource="http://www.w3.org/2001/XMLSchema#string"/>
  </owl:DatatypeProperty>
  <owl:DatatypeProperty rdf:about="http://example.org/onto/prop/google_spanner_database_kms_key_name">
    <rdfs:label>kms_key_name</rdfs:label>
    <rdfs:comment>Fully qualified name of the KMS key to use to encrypt this database. This key must exist
in the same location as the Spanner Database.</rdfs:comment>
    <rdfs:domain rdf:resource="http://example.org/onto/class/google_spanner_database"/>
    <rdfs:range rdf:resource="http://www.w3.org/2001/XMLSchema#string"/>
  </owl:DatatypeProperty>
  <owl:DatatypeProperty rdf:about="http://example.org/onto/prop/google_spanner_database_kms_key_names">
    <rdfs:label>kms_key_names</rdfs:label>
    <rdfs:comment>Fully qualified name of the KMS keys to use to encrypt this database. The keys must exist
in the same locations as the Spanner Database.</rdfs:comment>
    <rdfs:domain rdf:resource="http://example.org/onto/class/google_spanner_database"/>
    <rdfs:range rdf:resource="http://www.w3.org/2001/XMLSchema#string"/>
  </owl:DatatypeProperty>
  <owl:DatatypeProperty rdf:about="http://example.org/onto/prop/google_spanner_database_create">
    <rdfs:label>create</rdfs:label>
    <rdfs:domain rdf:resource="http://example.org/onto/class/google_spanner_database"/>
    <rdfs:range rdf:resource="http://www.w3.org/2001/XMLSchema#string"/>
  </owl:DatatypeProperty>
  <owl:DatatypeProperty rdf:about="http://example.org/onto/prop/google_spanner_database_delete">
    <rdfs:label>delete</rdfs:label>
    <rdfs:domain rdf:resource="http://example.org/onto/class/google_spanner_database"/>
    <rdfs:range rdf:resource="http://www.w3.org/2001/XMLSchema#string"/>
  </owl:DatatypeProperty>
  <owl:DatatypeProperty rdf:about="http://example.org/onto/prop/google_spanner_database_update">
    <rdfs:label>update</rdfs:label>
    <rdfs:domain rdf:resource="http://example.org/onto/class/google_spanner_database"/>
    <rdfs:range rdf:resource="http://www.w3.org/2001/XMLSchema#string"/>
  </owl:DatatypeProperty>
</rdf:RDF>
