<?xml version="1.0" encoding="UTF-8"?>
<rdf:RDF
  xmlns:rdf="http://www.w3.org/1999/02/22-rdf-syntax-ns#"
  xmlns:rdfs="http://www.w3.org/2000/01/rdf-schema#"
  xmlns:owl="http://www.w3.org/2002/07/owl#"
  xmlns:xsd="http://www.w3.org/2001/XMLSchema#"
  xml:base="http://example.org/onto/">
  <owl:Class rdf:about="http://example.org/onto/class/google_gke_hub_fleet">
    <rdfs:label>google_gke_hub_fleet</rdfs:label>
    <rdfs:comment>#
#     ***     AUTO GENERATED CODE    ***    Type: MMv1     ***
#
# ----------------------------------------------------------------------------
#
#     This code is generated by Magic Modules using the following:
#
#     Configuration: https:#github.com/GoogleCloudPlatform/magic-modules/tree/main/mmv1/products/gkehub2/Fleet.yaml
#     Template:      https:#github.com/GoogleCloudPlatform/magic-modules/tree/main/mmv1/templates/terraform/resource.html.markdown.tmpl
#
#     DO NOT EDIT this file directly. Any changes made to this file will be
#     overwritten during the next generation cycle.
#
# ----------------------------------------------------------------------------
subcategory: "GKEHub"
description: |-
  Fleet contains information about a group of clusters.
---</rdfs:comment>
  </owl:Class>
  <owl:DatatypeProperty rdf:about="http://example.org/onto/prop/google_gke_hub_fleet_create_time">
    <rdfs:label>create_time</rdfs:label>
    <rdfs:comment>The time the fleet was created, in RFC3339 text format.</rdfs:comment>
    <rdfs:domain rdf:resource="http://example.org/onto/class/google_gke_hub_fleet"/>
    <rdfs:range rdf:resource="http://www.w3.org/2001/XMLSchema#string"/>
  </owl:DatatypeProperty>
  <owl:DatatypeProperty rdf:about="http://example.org/onto/prop/google_gke_hub_fleet_delete_time">
    <rdfs:label>delete_time</rdfs:label>
    <rdfs:comment>The time the fleet was deleted, in RFC3339 text format.</rdfs:comment>
    <rdfs:domain rdf:resource="http://example.org/onto/class/google_gke_hub_fleet"/>
    <rdfs:range rdf:resource="http://www.w3.org/2001/XMLSchema#string"/>
  </owl:DatatypeProperty>
  <owl:DatatypeProperty rdf:about="http://example.org/onto/prop/google_gke_hub_fleet_display_name">
    <rdfs:label>display_name</rdfs:label>
    <rdfs:comment>A user-assigned display name of the Fleet. When present, it must be between 4 to 30 characters.
Allowed characters are: lowercase and uppercase letters, numbers, hyphen, single-quote, double-quote, space, and exclamation point.</rdfs:comment>
    <rdfs:domain rdf:resource="http://example.org/onto/class/google_gke_hub_fleet"/>
    <rdfs:range rdf:resource="http://www.w3.org/2001/XMLSchema#string"/>
  </owl:DatatypeProperty>
  <owl:DatatypeProperty rdf:about="http://example.org/onto/prop/google_gke_hub_fleet_id">
    <rdfs:label>id</rdfs:label>
    <rdfs:domain rdf:resource="http://example.org/onto/class/google_gke_hub_fleet"/>
    <rdfs:range rdf:resource="http://www.w3.org/2001/XMLSchema#string"/>
  </owl:DatatypeProperty>
  <owl:DatatypeProperty rdf:about="http://example.org/onto/prop/google_gke_hub_fleet_project">
    <rdfs:label>project</rdfs:label>
    <rdfs:domain rdf:resource="http://example.org/onto/class/google_gke_hub_fleet"/>
    <rdfs:range rdf:resource="http://www.w3.org/2001/XMLSchema#string"/>
  </owl:DatatypeProperty>
  <owl:DatatypeProperty rdf:about="http://example.org/onto/prop/google_gke_hub_fleet_state">
    <rdfs:label>state</rdfs:label>
    <rdfs:comment>The state of the fleet resource.</rdfs:comment>
    <rdfs:domain rdf:resource="http://example.org/onto/class/google_gke_hub_fleet"/>
    <rdfs:range rdf:resource="http://www.w3.org/2001/XMLSchema#string"/>
  </owl:DatatypeProperty>
  <owl:DatatypeProperty rdf:about="http://example.org/onto/prop/google_gke_hub_fleet_uid">
    <rdfs:label>uid</rdfs:label>
    <rdfs:comment>Google-generated UUID for this resource. This is unique across all
Fleet resources. If a Fleet resource is deleted and another
resource with the same name is created, it gets a different uid.</rdfs:comment>
    <rdfs:domain rdf:resource="http://example.org/onto/class/google_gke_hub_fleet"/>
    <rdfs:range rdf:resource="http://www.w3.org/2001/XMLSchema#string"/>
  </owl:DatatypeProperty>
  <owl:DatatypeProperty rdf:about="http://example.org/onto/prop/google_gke_hub_fleet_update_time">
    <rdfs:label>update_time</rdfs:label>
    <rdfs:comment>The time the fleet was last updated, in RFC3339 text format.</rdfs:comment>
    <rdfs:domain rdf:resource="http://example.org/onto/class/google_gke_hub_fleet"/>
    <rdfs:range rdf:resource="http://www.w3.org/2001/XMLSchema#string"/>
  </owl:DatatypeProperty>
  <owl:DatatypeProperty rdf:about="http://example.org/onto/prop/google_gke_hub_fleet_evaluation_mode">
    <rdfs:label>evaluation_mode</rdfs:label>
    <rdfs:comment>Mode of operation for binauthz policy evaluation. Possible values: ["DISABLED", "POLICY_BINDINGS"]</rdfs:comment>
    <rdfs:domain rdf:resource="http://example.org/onto/class/google_gke_hub_fleet"/>
    <rdfs:range rdf:resource="http://www.w3.org/2001/XMLSchema#string"/>
  </owl:DatatypeProperty>
  <owl:DatatypeProperty rdf:about="http://example.org/onto/prop/google_gke_hub_fleet_name">
    <rdfs:label>name</rdfs:label>
    <rdfs:comment>The relative resource name of the binauthz platform policy to audit. GKE
platform policies have the following format:
'projects/{project_number}/platforms/gke/policies/{policy_id}'.</rdfs:comment>
    <rdfs:domain rdf:resource="http://example.org/onto/class/google_gke_hub_fleet"/>
    <rdfs:range rdf:resource="http://www.w3.org/2001/XMLSchema#string"/>
  </owl:DatatypeProperty>
  <owl:DatatypeProperty rdf:about="http://example.org/onto/prop/google_gke_hub_fleet_mode">
    <rdfs:label>mode</rdfs:label>
    <rdfs:comment>Sets which mode to use for Security Posture features. Possible values: ["DISABLED", "BASIC", "ENTERPRISE"]</rdfs:comment>
    <rdfs:domain rdf:resource="http://example.org/onto/class/google_gke_hub_fleet"/>
    <rdfs:range rdf:resource="http://www.w3.org/2001/XMLSchema#string"/>
  </owl:DatatypeProperty>
  <owl:DatatypeProperty rdf:about="http://example.org/onto/prop/google_gke_hub_fleet_vulnerability_mode">
    <rdfs:label>vulnerability_mode</rdfs:label>
    <rdfs:comment>Sets which mode to use for vulnerability scanning. Possible values: ["VULNERABILITY_DISABLED", "VULNERABILITY_BASIC", "VULNERABILITY_ENTERPRISE"]</rdfs:comment>
    <rdfs:domain rdf:resource="http://example.org/onto/class/google_gke_hub_fleet"/>
    <rdfs:range rdf:resource="http://www.w3.org/2001/XMLSchema#string"/>
  </owl:DatatypeProperty>
  <owl:DatatypeProperty rdf:about="http://example.org/onto/prop/google_gke_hub_fleet_create">
    <rdfs:label>create</rdfs:label>
    <rdfs:domain rdf:resource="http://example.org/onto/class/google_gke_hub_fleet"/>
    <rdfs:range rdf:resource="http://www.w3.org/2001/XMLSchema#string"/>
  </owl:DatatypeProperty>
  <owl:DatatypeProperty rdf:about="http://example.org/onto/prop/google_gke_hub_fleet_delete">
    <rdfs:label>delete</rdfs:label>
    <rdfs:domain rdf:resource="http://example.org/onto/class/google_gke_hub_fleet"/>
    <rdfs:range rdf:resource="http://www.w3.org/2001/XMLSchema#string"/>
  </owl:DatatypeProperty>
  <owl:DatatypeProperty rdf:about="http://example.org/onto/prop/google_gke_hub_fleet_update">
    <rdfs:label>update</rdfs:label>
    <rdfs:domain rdf:resource="http://example.org/onto/class/google_gke_hub_fleet"/>
    <rdfs:range rdf:resource="http://www.w3.org/2001/XMLSchema#string"/>
  </owl:DatatypeProperty>
</rdf:RDF>
