<?xml version="1.0" encoding="UTF-8"?>
<rdf:RDF
  xmlns:rdf="http://www.w3.org/1999/02/22-rdf-syntax-ns#"
  xmlns:rdfs="http://www.w3.org/2000/01/rdf-schema#"
  xmlns:owl="http://www.w3.org/2002/07/owl#"
  xmlns:xsd="http://www.w3.org/2001/XMLSchema#"
  xml:base="http://example.org/onto/">
  <owl:Class rdf:about="http://example.org/onto/class/google_gke_hub_feature_membership">
    <rdfs:label>google_gke_hub_feature_membership</rdfs:label>
    <rdfs:comment>#
#     ***     AUTO GENERATED CODE    ***    Type: Handwritten     ***
#
# ----------------------------------------------------------------------------
#
#     This code is generated by Magic Modules using the following:
#
#     Source file: https://github.com/GoogleCloudPlatform/magic-modules/tree/main/mmv1/third_party/terraform/website/docs/r/gke_hub_feature_membership.html.markdown
#
#     DO NOT EDIT this file directly. Any changes made to this file will be
#     overwritten during the next generation cycle.
#
# ----------------------------------------------------------------------------
subcategory: "GKEHub"
description: |-
  Contains information about a GKEHub Feature Memberships.
---</rdfs:comment>
  </owl:Class>
  <owl:DatatypeProperty rdf:about="http://example.org/onto/prop/google_gke_hub_feature_membership_feature">
    <rdfs:label>feature</rdfs:label>
    <rdfs:comment>The name of the feature</rdfs:comment>
    <rdfs:domain rdf:resource="http://example.org/onto/class/google_gke_hub_feature_membership"/>
    <rdfs:range rdf:resource="http://www.w3.org/2001/XMLSchema#string"/>
  </owl:DatatypeProperty>
  <owl:DatatypeProperty rdf:about="http://example.org/onto/prop/google_gke_hub_feature_membership_id">
    <rdfs:label>id</rdfs:label>
    <rdfs:domain rdf:resource="http://example.org/onto/class/google_gke_hub_feature_membership"/>
    <rdfs:range rdf:resource="http://www.w3.org/2001/XMLSchema#string"/>
  </owl:DatatypeProperty>
  <owl:DatatypeProperty rdf:about="http://example.org/onto/prop/google_gke_hub_feature_membership_location">
    <rdfs:label>location</rdfs:label>
    <rdfs:comment>The location of the feature</rdfs:comment>
    <rdfs:domain rdf:resource="http://example.org/onto/class/google_gke_hub_feature_membership"/>
    <rdfs:range rdf:resource="http://www.w3.org/2001/XMLSchema#string"/>
  </owl:DatatypeProperty>
  <owl:DatatypeProperty rdf:about="http://example.org/onto/prop/google_gke_hub_feature_membership_membership">
    <rdfs:label>membership</rdfs:label>
    <rdfs:comment>The name of the membership</rdfs:comment>
    <rdfs:domain rdf:resource="http://example.org/onto/class/google_gke_hub_feature_membership"/>
    <rdfs:range rdf:resource="http://www.w3.org/2001/XMLSchema#string"/>
  </owl:DatatypeProperty>
  <owl:DatatypeProperty rdf:about="http://example.org/onto/prop/google_gke_hub_feature_membership_membership_location">
    <rdfs:label>membership_location</rdfs:label>
    <rdfs:comment>The location of the membership</rdfs:comment>
    <rdfs:domain rdf:resource="http://example.org/onto/class/google_gke_hub_feature_membership"/>
    <rdfs:range rdf:resource="http://www.w3.org/2001/XMLSchema#string"/>
  </owl:DatatypeProperty>
  <owl:DatatypeProperty rdf:about="http://example.org/onto/prop/google_gke_hub_feature_membership_project">
    <rdfs:label>project</rdfs:label>
    <rdfs:comment>The project of the feature</rdfs:comment>
    <rdfs:domain rdf:resource="http://example.org/onto/class/google_gke_hub_feature_membership"/>
    <rdfs:range rdf:resource="http://www.w3.org/2001/XMLSchema#string"/>
  </owl:DatatypeProperty>
  <owl:DatatypeProperty rdf:about="http://example.org/onto/prop/google_gke_hub_feature_membership_management">
    <rdfs:label>management</rdfs:label>
    <rdfs:comment>Set this field to MANAGEMENT_AUTOMATIC to enable Config Sync auto-upgrades, and set this field to MANAGEMENT_MANUAL or MANAGEMENT_UNSPECIFIED to disable Config Sync auto-upgrades.</rdfs:comment>
    <rdfs:domain rdf:resource="http://example.org/onto/class/google_gke_hub_feature_membership"/>
    <rdfs:range rdf:resource="http://www.w3.org/2001/XMLSchema#string"/>
  </owl:DatatypeProperty>
  <owl:DatatypeProperty rdf:about="http://example.org/onto/prop/google_gke_hub_feature_membership_version">
    <rdfs:label>version</rdfs:label>
    <rdfs:comment>Optional. Version of ACM to install. Defaults to the latest version.</rdfs:comment>
    <rdfs:domain rdf:resource="http://example.org/onto/class/google_gke_hub_feature_membership"/>
    <rdfs:range rdf:resource="http://www.w3.org/2001/XMLSchema#string"/>
  </owl:DatatypeProperty>
  <owl:DatatypeProperty rdf:about="http://example.org/onto/prop/google_gke_hub_feature_membership_enabled">
    <rdfs:label>enabled</rdfs:label>
    <rdfs:comment>Enables the installation of ConfigSync. If set to true, ConfigSync resources will be created and the other ConfigSync fields will be applied if exist. If set to false, all other ConfigSync fields will be ignored, ConfigSync resources will be deleted. If omitted, ConfigSync resources will be managed depends on the presence of the git or oci field.</rdfs:comment>
    <rdfs:domain rdf:resource="http://example.org/onto/class/google_gke_hub_feature_membership"/>
    <rdfs:range rdf:resource="http://www.w3.org/2001/XMLSchema#string"/>
  </owl:DatatypeProperty>
  <owl:DatatypeProperty rdf:about="http://example.org/onto/prop/google_gke_hub_feature_membership_metrics_gcp_service_account_email">
    <rdfs:label>metrics_gcp_service_account_email</rdfs:label>
    <rdfs:comment>Deprecated: If Workload Identity Federation for GKE is enabled, Google Cloud Service Account is no longer needed for exporting Config Sync metrics: https://cloud.google.com/kubernetes-engine/enterprise/config-sync/docs/how-to/monitor-config-sync-cloud-monitoring#custom-monitoring.</rdfs:comment>
    <rdfs:domain rdf:resource="http://example.org/onto/class/google_gke_hub_feature_membership"/>
    <rdfs:range rdf:resource="http://www.w3.org/2001/XMLSchema#string"/>
  </owl:DatatypeProperty>
  <owl:DatatypeProperty rdf:about="http://example.org/onto/prop/google_gke_hub_feature_membership_prevent_drift">
    <rdfs:label>prevent_drift</rdfs:label>
    <rdfs:comment>Set to true to enable the Config Sync admission webhook to prevent drifts. If set to `false`, disables the Config Sync admission webhook and does not prevent drifts.</rdfs:comment>
    <rdfs:domain rdf:resource="http://example.org/onto/class/google_gke_hub_feature_membership"/>
    <rdfs:range rdf:resource="http://www.w3.org/2001/XMLSchema#string"/>
  </owl:DatatypeProperty>
  <owl:DatatypeProperty rdf:about="http://example.org/onto/prop/google_gke_hub_feature_membership_source_format">
    <rdfs:label>source_format</rdfs:label>
    <rdfs:comment>Specifies whether the Config Sync Repo is in "hierarchical" or "unstructured" mode.</rdfs:comment>
    <rdfs:domain rdf:resource="http://example.org/onto/class/google_gke_hub_feature_membership"/>
    <rdfs:range rdf:resource="http://www.w3.org/2001/XMLSchema#string"/>
  </owl:DatatypeProperty>
  <owl:DatatypeProperty rdf:about="http://example.org/onto/prop/google_gke_hub_feature_membership_stop_syncing">
    <rdfs:label>stop_syncing</rdfs:label>
    <rdfs:comment>Set to true to stop syncing configs for a single cluster. Default: false.</rdfs:comment>
    <rdfs:domain rdf:resource="http://example.org/onto/class/google_gke_hub_feature_membership"/>
    <rdfs:range rdf:resource="http://www.w3.org/2001/XMLSchema#string"/>
  </owl:DatatypeProperty>
  <owl:DatatypeProperty rdf:about="http://example.org/onto/prop/google_gke_hub_feature_membership_deployment_name">
    <rdfs:label>deployment_name</rdfs:label>
    <rdfs:comment>The name of the Deployment.</rdfs:comment>
    <rdfs:domain rdf:resource="http://example.org/onto/class/google_gke_hub_feature_membership"/>
    <rdfs:range rdf:resource="http://www.w3.org/2001/XMLSchema#string"/>
  </owl:DatatypeProperty>
  <owl:DatatypeProperty rdf:about="http://example.org/onto/prop/google_gke_hub_feature_membership_deployment_namespace">
    <rdfs:label>deployment_namespace</rdfs:label>
    <rdfs:comment>The namespace of the Deployment.</rdfs:comment>
    <rdfs:domain rdf:resource="http://example.org/onto/class/google_gke_hub_feature_membership"/>
    <rdfs:range rdf:resource="http://www.w3.org/2001/XMLSchema#string"/>
  </owl:DatatypeProperty>
  <owl:DatatypeProperty rdf:about="http://example.org/onto/prop/google_gke_hub_feature_membership_container_name">
    <rdfs:label>container_name</rdfs:label>
    <rdfs:comment>The name of the container.</rdfs:comment>
    <rdfs:domain rdf:resource="http://example.org/onto/class/google_gke_hub_feature_membership"/>
    <rdfs:range rdf:resource="http://www.w3.org/2001/XMLSchema#string"/>
  </owl:DatatypeProperty>
  <owl:DatatypeProperty rdf:about="http://example.org/onto/prop/google_gke_hub_feature_membership_cpu_limit">
    <rdfs:label>cpu_limit</rdfs:label>
    <rdfs:comment>The CPU limit of the container.</rdfs:comment>
    <rdfs:domain rdf:resource="http://example.org/onto/class/google_gke_hub_feature_membership"/>
    <rdfs:range rdf:resource="http://www.w3.org/2001/XMLSchema#string"/>
  </owl:DatatypeProperty>
  <owl:DatatypeProperty rdf:about="http://example.org/onto/prop/google_gke_hub_feature_membership_cpu_request">
    <rdfs:label>cpu_request</rdfs:label>
    <rdfs:comment>The CPU request of the container.</rdfs:comment>
    <rdfs:domain rdf:resource="http://example.org/onto/class/google_gke_hub_feature_membership"/>
    <rdfs:range rdf:resource="http://www.w3.org/2001/XMLSchema#string"/>
  </owl:DatatypeProperty>
  <owl:DatatypeProperty rdf:about="http://example.org/onto/prop/google_gke_hub_feature_membership_memory_limit">
    <rdfs:label>memory_limit</rdfs:label>
    <rdfs:comment>The memory limit of the container.</rdfs:comment>
    <rdfs:domain rdf:resource="http://example.org/onto/class/google_gke_hub_feature_membership"/>
    <rdfs:range rdf:resource="http://www.w3.org/2001/XMLSchema#string"/>
  </owl:DatatypeProperty>
  <owl:DatatypeProperty rdf:about="http://example.org/onto/prop/google_gke_hub_feature_membership_memory_request">
    <rdfs:label>memory_request</rdfs:label>
    <rdfs:comment>The memory request of the container.</rdfs:comment>
    <rdfs:domain rdf:resource="http://example.org/onto/class/google_gke_hub_feature_membership"/>
    <rdfs:range rdf:resource="http://www.w3.org/2001/XMLSchema#string"/>
  </owl:DatatypeProperty>
  <owl:DatatypeProperty rdf:about="http://example.org/onto/prop/google_gke_hub_feature_membership_gcp_service_account_email">
    <rdfs:label>gcp_service_account_email</rdfs:label>
    <rdfs:comment>The GCP Service Account Email used for auth when secretType is gcpServiceAccount.</rdfs:comment>
    <rdfs:domain rdf:resource="http://example.org/onto/class/google_gke_hub_feature_membership"/>
    <rdfs:range rdf:resource="http://www.w3.org/2001/XMLSchema#string"/>
  </owl:DatatypeProperty>
  <owl:DatatypeProperty rdf:about="http://example.org/onto/prop/google_gke_hub_feature_membership_https_proxy">
    <rdfs:label>https_proxy</rdfs:label>
    <rdfs:comment>URL for the HTTPS proxy to be used when communicating with the Git repo.</rdfs:comment>
    <rdfs:domain rdf:resource="http://example.org/onto/class/google_gke_hub_feature_membership"/>
    <rdfs:range rdf:resource="http://www.w3.org/2001/XMLSchema#string"/>
  </owl:DatatypeProperty>
  <owl:DatatypeProperty rdf:about="http://example.org/onto/prop/google_gke_hub_feature_membership_policy_dir">
    <rdfs:label>policy_dir</rdfs:label>
    <rdfs:comment>The path within the Git repository that represents the top level of the repo to sync. Default: the root directory of the repository.</rdfs:comment>
    <rdfs:domain rdf:resource="http://example.org/onto/class/google_gke_hub_feature_membership"/>
    <rdfs:range rdf:resource="http://www.w3.org/2001/XMLSchema#string"/>
  </owl:DatatypeProperty>
  <owl:DatatypeProperty rdf:about="http://example.org/onto/prop/google_gke_hub_feature_membership_secret_type">
    <rdfs:label>secret_type</rdfs:label>
    <rdfs:comment>Type of secret configured for access to the Git repo. Must be one of ssh, cookiefile, gcenode, token, gcpserviceaccount or none. The validation of this is case-sensitive.</rdfs:comment>
    <rdfs:domain rdf:resource="http://example.org/onto/class/google_gke_hub_feature_membership"/>
    <rdfs:range rdf:resource="http://www.w3.org/2001/XMLSchema#string"/>
  </owl:DatatypeProperty>
  <owl:DatatypeProperty rdf:about="http://example.org/onto/prop/google_gke_hub_feature_membership_sync_branch">
    <rdfs:label>sync_branch</rdfs:label>
    <rdfs:comment>The branch of the repository to sync from. Default: master.</rdfs:comment>
    <rdfs:domain rdf:resource="http://example.org/onto/class/google_gke_hub_feature_membership"/>
    <rdfs:range rdf:resource="http://www.w3.org/2001/XMLSchema#string"/>
  </owl:DatatypeProperty>
  <owl:DatatypeProperty rdf:about="http://example.org/onto/prop/google_gke_hub_feature_membership_sync_repo">
    <rdfs:label>sync_repo</rdfs:label>
    <rdfs:comment>The URL of the Git repository to use as the source of truth.</rdfs:comment>
    <rdfs:domain rdf:resource="http://example.org/onto/class/google_gke_hub_feature_membership"/>
    <rdfs:range rdf:resource="http://www.w3.org/2001/XMLSchema#string"/>
  </owl:DatatypeProperty>
  <owl:DatatypeProperty rdf:about="http://example.org/onto/prop/google_gke_hub_feature_membership_sync_rev">
    <rdfs:label>sync_rev</rdfs:label>
    <rdfs:comment>Git revision (tag or hash) to check out. Default HEAD.</rdfs:comment>
    <rdfs:domain rdf:resource="http://example.org/onto/class/google_gke_hub_feature_membership"/>
    <rdfs:range rdf:resource="http://www.w3.org/2001/XMLSchema#string"/>
  </owl:DatatypeProperty>
  <owl:DatatypeProperty rdf:about="http://example.org/onto/prop/google_gke_hub_feature_membership_sync_wait_secs">
    <rdfs:label>sync_wait_secs</rdfs:label>
    <rdfs:comment>Period in seconds between consecutive syncs. Default: 15.</rdfs:comment>
    <rdfs:domain rdf:resource="http://example.org/onto/class/google_gke_hub_feature_membership"/>
    <rdfs:range rdf:resource="http://www.w3.org/2001/XMLSchema#string"/>
  </owl:DatatypeProperty>
  <owl:DatatypeProperty rdf:about="http://example.org/onto/prop/google_gke_hub_feature_membership_gcp_service_account_email">
    <rdfs:label>gcp_service_account_email</rdfs:label>
    <rdfs:comment>The GCP Service Account Email used for auth when secret_type is gcpserviceaccount.</rdfs:comment>
    <rdfs:domain rdf:resource="http://example.org/onto/class/google_gke_hub_feature_membership"/>
    <rdfs:range rdf:resource="http://www.w3.org/2001/XMLSchema#string"/>
  </owl:DatatypeProperty>
  <owl:DatatypeProperty rdf:about="http://example.org/onto/prop/google_gke_hub_feature_membership_policy_dir">
    <rdfs:label>policy_dir</rdfs:label>
    <rdfs:comment>The absolute path of the directory that contains the local resources. Default: the root directory of the image.</rdfs:comment>
    <rdfs:domain rdf:resource="http://example.org/onto/class/google_gke_hub_feature_membership"/>
    <rdfs:range rdf:resource="http://www.w3.org/2001/XMLSchema#string"/>
  </owl:DatatypeProperty>
  <owl:DatatypeProperty rdf:about="http://example.org/onto/prop/google_gke_hub_feature_membership_secret_type">
    <rdfs:label>secret_type</rdfs:label>
    <rdfs:comment>Type of secret configured for access to the OCI Image. Must be one of gcenode, gcpserviceaccount or none. The validation of this is case-sensitive.</rdfs:comment>
    <rdfs:domain rdf:resource="http://example.org/onto/class/google_gke_hub_feature_membership"/>
    <rdfs:range rdf:resource="http://www.w3.org/2001/XMLSchema#string"/>
  </owl:DatatypeProperty>
  <owl:DatatypeProperty rdf:about="http://example.org/onto/prop/google_gke_hub_feature_membership_sync_repo">
    <rdfs:label>sync_repo</rdfs:label>
    <rdfs:comment>The OCI image repository URL for the package to sync from. e.g. LOCATION-docker.pkg.dev/PROJECT_ID/REPOSITORY_NAME/PACKAGE_NAME.</rdfs:comment>
    <rdfs:domain rdf:resource="http://example.org/onto/class/google_gke_hub_feature_membership"/>
    <rdfs:range rdf:resource="http://www.w3.org/2001/XMLSchema#string"/>
  </owl:DatatypeProperty>
  <owl:DatatypeProperty rdf:about="http://example.org/onto/prop/google_gke_hub_feature_membership_sync_wait_secs">
    <rdfs:label>sync_wait_secs</rdfs:label>
    <rdfs:comment>Period in seconds(int64 format) between consecutive syncs. Default: 15.</rdfs:comment>
    <rdfs:domain rdf:resource="http://example.org/onto/class/google_gke_hub_feature_membership"/>
    <rdfs:range rdf:resource="http://www.w3.org/2001/XMLSchema#string"/>
  </owl:DatatypeProperty>
  <owl:DatatypeProperty rdf:about="http://example.org/onto/prop/google_gke_hub_feature_membership_enable_hierarchical_resource_quota">
    <rdfs:label>enable_hierarchical_resource_quota</rdfs:label>
    <rdfs:comment>Whether hierarchical resource quota is enabled in this cluster.</rdfs:comment>
    <rdfs:domain rdf:resource="http://example.org/onto/class/google_gke_hub_feature_membership"/>
    <rdfs:range rdf:resource="http://www.w3.org/2001/XMLSchema#string"/>
  </owl:DatatypeProperty>
  <owl:DatatypeProperty rdf:about="http://example.org/onto/prop/google_gke_hub_feature_membership_enable_pod_tree_labels">
    <rdfs:label>enable_pod_tree_labels</rdfs:label>
    <rdfs:comment>Whether pod tree labels are enabled in this cluster.</rdfs:comment>
    <rdfs:domain rdf:resource="http://example.org/onto/class/google_gke_hub_feature_membership"/>
    <rdfs:range rdf:resource="http://www.w3.org/2001/XMLSchema#string"/>
  </owl:DatatypeProperty>
  <owl:DatatypeProperty rdf:about="http://example.org/onto/prop/google_gke_hub_feature_membership_enabled">
    <rdfs:label>enabled</rdfs:label>
    <rdfs:comment>**DEPRECATED** Configuring Hierarchy Controller through the configmanagement feature is no longer recommended. Use https://github.com/kubernetes-sigs/hierarchical-namespaces instead.</rdfs:comment>
    <rdfs:domain rdf:resource="http://example.org/onto/class/google_gke_hub_feature_membership"/>
    <rdfs:range rdf:resource="http://www.w3.org/2001/XMLSchema#string"/>
  </owl:DatatypeProperty>
  <owl:DatatypeProperty rdf:about="http://example.org/onto/prop/google_gke_hub_feature_membership_audit_interval_seconds">
    <rdfs:label>audit_interval_seconds</rdfs:label>
    <rdfs:comment>Sets the interval for Policy Controller Audit Scans (in seconds). When set to 0, this disables audit functionality altogether.</rdfs:comment>
    <rdfs:domain rdf:resource="http://example.org/onto/class/google_gke_hub_feature_membership"/>
    <rdfs:range rdf:resource="http://www.w3.org/2001/XMLSchema#string"/>
  </owl:DatatypeProperty>
  <owl:DatatypeProperty rdf:about="http://example.org/onto/prop/google_gke_hub_feature_membership_enabled">
    <rdfs:label>enabled</rdfs:label>
    <rdfs:comment>Enables the installation of Policy Controller. If false, the rest of PolicyController fields take no effect.</rdfs:comment>
    <rdfs:domain rdf:resource="http://example.org/onto/class/google_gke_hub_feature_membership"/>
    <rdfs:range rdf:resource="http://www.w3.org/2001/XMLSchema#string"/>
  </owl:DatatypeProperty>
  <owl:DatatypeProperty rdf:about="http://example.org/onto/prop/google_gke_hub_feature_membership_exemptable_namespaces">
    <rdfs:label>exemptable_namespaces</rdfs:label>
    <rdfs:comment>The set of namespaces that are excluded from Policy Controller checks. Namespaces do not need to currently exist on the cluster.</rdfs:comment>
    <rdfs:domain rdf:resource="http://example.org/onto/class/google_gke_hub_feature_membership"/>
    <rdfs:range rdf:resource="http://www.w3.org/2001/XMLSchema#string"/>
  </owl:DatatypeProperty>
  <owl:DatatypeProperty rdf:about="http://example.org/onto/prop/google_gke_hub_feature_membership_log_denies_enabled">
    <rdfs:label>log_denies_enabled</rdfs:label>
    <rdfs:comment>Logs all denies and dry run failures.</rdfs:comment>
    <rdfs:domain rdf:resource="http://example.org/onto/class/google_gke_hub_feature_membership"/>
    <rdfs:range rdf:resource="http://www.w3.org/2001/XMLSchema#string"/>
  </owl:DatatypeProperty>
  <owl:DatatypeProperty rdf:about="http://example.org/onto/prop/google_gke_hub_feature_membership_mutation_enabled">
    <rdfs:label>mutation_enabled</rdfs:label>
    <rdfs:comment>Enable or disable mutation in policy controller. If true, mutation CRDs, webhook and controller deployment will be deployed to the cluster.</rdfs:comment>
    <rdfs:domain rdf:resource="http://example.org/onto/class/google_gke_hub_feature_membership"/>
    <rdfs:range rdf:resource="http://www.w3.org/2001/XMLSchema#string"/>
  </owl:DatatypeProperty>
  <owl:DatatypeProperty rdf:about="http://example.org/onto/prop/google_gke_hub_feature_membership_referential_rules_enabled">
    <rdfs:label>referential_rules_enabled</rdfs:label>
    <rdfs:comment>Enables the ability to use Constraint Templates that reference to objects other than the object currently being evaluated.</rdfs:comment>
    <rdfs:domain rdf:resource="http://example.org/onto/class/google_gke_hub_feature_membership"/>
    <rdfs:range rdf:resource="http://www.w3.org/2001/XMLSchema#string"/>
  </owl:DatatypeProperty>
  <owl:DatatypeProperty rdf:about="http://example.org/onto/prop/google_gke_hub_feature_membership_template_library_installed">
    <rdfs:label>template_library_installed</rdfs:label>
    <rdfs:comment>Installs the default template library along with Policy Controller.</rdfs:comment>
    <rdfs:domain rdf:resource="http://example.org/onto/class/google_gke_hub_feature_membership"/>
    <rdfs:range rdf:resource="http://www.w3.org/2001/XMLSchema#string"/>
  </owl:DatatypeProperty>
  <owl:DatatypeProperty rdf:about="http://example.org/onto/prop/google_gke_hub_feature_membership_backends">
    <rdfs:label>backends</rdfs:label>
    <rdfs:comment>Specifies the list of backends Policy Controller will export to. Specifying an empty value `[]` disables metrics export.</rdfs:comment>
    <rdfs:domain rdf:resource="http://example.org/onto/class/google_gke_hub_feature_membership"/>
    <rdfs:range rdf:resource="http://www.w3.org/2001/XMLSchema#string"/>
  </owl:DatatypeProperty>
  <owl:DatatypeProperty rdf:about="http://example.org/onto/prop/google_gke_hub_feature_membership_control_plane">
    <rdfs:label>control_plane</rdfs:label>
    <rdfs:comment>**DEPRECATED** Whether to automatically manage Service Mesh control planes. Possible values: CONTROL_PLANE_MANAGEMENT_UNSPECIFIED, AUTOMATIC, MANUAL</rdfs:comment>
    <rdfs:domain rdf:resource="http://example.org/onto/class/google_gke_hub_feature_membership"/>
    <rdfs:range rdf:resource="http://www.w3.org/2001/XMLSchema#string"/>
  </owl:DatatypeProperty>
  <owl:DatatypeProperty rdf:about="http://example.org/onto/prop/google_gke_hub_feature_membership_management">
    <rdfs:label>management</rdfs:label>
    <rdfs:comment>Whether to automatically manage Service Mesh. Possible values: MANAGEMENT_UNSPECIFIED, MANAGEMENT_AUTOMATIC, MANAGEMENT_MANUAL</rdfs:comment>
    <rdfs:domain rdf:resource="http://example.org/onto/class/google_gke_hub_feature_membership"/>
    <rdfs:range rdf:resource="http://www.w3.org/2001/XMLSchema#string"/>
  </owl:DatatypeProperty>
  <owl:DatatypeProperty rdf:about="http://example.org/onto/prop/google_gke_hub_feature_membership_version">
    <rdfs:label>version</rdfs:label>
    <rdfs:comment>Optional. Version of Policy Controller to install. Defaults to the latest version.</rdfs:comment>
    <rdfs:domain rdf:resource="http://example.org/onto/class/google_gke_hub_feature_membership"/>
    <rdfs:range rdf:resource="http://www.w3.org/2001/XMLSchema#string"/>
  </owl:DatatypeProperty>
  <owl:DatatypeProperty rdf:about="http://example.org/onto/prop/google_gke_hub_feature_membership_audit_interval_seconds">
    <rdfs:label>audit_interval_seconds</rdfs:label>
    <rdfs:comment>Sets the interval for Policy Controller Audit Scans (in seconds). When set to 0, this disables audit functionality altogether.</rdfs:comment>
    <rdfs:domain rdf:resource="http://example.org/onto/class/google_gke_hub_feature_membership"/>
    <rdfs:range rdf:resource="http://www.w3.org/2001/XMLSchema#string"/>
  </owl:DatatypeProperty>
  <owl:DatatypeProperty rdf:about="http://example.org/onto/prop/google_gke_hub_feature_membership_constraint_violation_limit">
    <rdfs:label>constraint_violation_limit</rdfs:label>
    <rdfs:comment>The maximum number of audit violations to be stored in a constraint. If not set, the internal default of 20 will be used.</rdfs:comment>
    <rdfs:domain rdf:resource="http://example.org/onto/class/google_gke_hub_feature_membership"/>
    <rdfs:range rdf:resource="http://www.w3.org/2001/XMLSchema#string"/>
  </owl:DatatypeProperty>
  <owl:DatatypeProperty rdf:about="http://example.org/onto/prop/google_gke_hub_feature_membership_exemptable_namespaces">
    <rdfs:label>exemptable_namespaces</rdfs:label>
    <rdfs:comment>The set of namespaces that are excluded from Policy Controller checks. Namespaces do not need to currently exist on the cluster.</rdfs:comment>
    <rdfs:domain rdf:resource="http://example.org/onto/class/google_gke_hub_feature_membership"/>
    <rdfs:range rdf:resource="http://www.w3.org/2001/XMLSchema#string"/>
  </owl:DatatypeProperty>
  <owl:DatatypeProperty rdf:about="http://example.org/onto/prop/google_gke_hub_feature_membership_install_spec">
    <rdfs:label>install_spec</rdfs:label>
    <rdfs:comment>Configures the mode of the Policy Controller installation. Possible values: INSTALL_SPEC_UNSPECIFIED, INSTALL_SPEC_NOT_INSTALLED, INSTALL_SPEC_ENABLED, INSTALL_SPEC_SUSPENDED, INSTALL_SPEC_DETACHED</rdfs:comment>
    <rdfs:domain rdf:resource="http://example.org/onto/class/google_gke_hub_feature_membership"/>
    <rdfs:range rdf:resource="http://www.w3.org/2001/XMLSchema#string"/>
  </owl:DatatypeProperty>
  <owl:DatatypeProperty rdf:about="http://example.org/onto/prop/google_gke_hub_feature_membership_log_denies_enabled">
    <rdfs:label>log_denies_enabled</rdfs:label>
    <rdfs:comment>Logs all denies and dry run failures.</rdfs:comment>
    <rdfs:domain rdf:resource="http://example.org/onto/class/google_gke_hub_feature_membership"/>
    <rdfs:range rdf:resource="http://www.w3.org/2001/XMLSchema#string"/>
  </owl:DatatypeProperty>
  <owl:DatatypeProperty rdf:about="http://example.org/onto/prop/google_gke_hub_feature_membership_mutation_enabled">
    <rdfs:label>mutation_enabled</rdfs:label>
    <rdfs:comment>Enables the ability to mutate resources using Policy Controller.</rdfs:comment>
    <rdfs:domain rdf:resource="http://example.org/onto/class/google_gke_hub_feature_membership"/>
    <rdfs:range rdf:resource="http://www.w3.org/2001/XMLSchema#string"/>
  </owl:DatatypeProperty>
  <owl:DatatypeProperty rdf:about="http://example.org/onto/prop/google_gke_hub_feature_membership_referential_rules_enabled">
    <rdfs:label>referential_rules_enabled</rdfs:label>
    <rdfs:comment>Enables the ability to use Constraint Templates that reference to objects other than the object currently being evaluated.</rdfs:comment>
    <rdfs:domain rdf:resource="http://example.org/onto/class/google_gke_hub_feature_membership"/>
    <rdfs:range rdf:resource="http://www.w3.org/2001/XMLSchema#string"/>
  </owl:DatatypeProperty>
  <owl:DatatypeProperty rdf:about="http://example.org/onto/prop/google_gke_hub_feature_membership_component_name">
    <rdfs:label>component_name</rdfs:label>
    <rdfs:comment>The name for the key in the map for which this object is mapped to in the API</rdfs:comment>
    <rdfs:domain rdf:resource="http://example.org/onto/class/google_gke_hub_feature_membership"/>
    <rdfs:range rdf:resource="http://www.w3.org/2001/XMLSchema#string"/>
  </owl:DatatypeProperty>
  <owl:DatatypeProperty rdf:about="http://example.org/onto/prop/google_gke_hub_feature_membership_pod_affinity">
    <rdfs:label>pod_affinity</rdfs:label>
    <rdfs:comment>Pod affinity configuration. Possible values: AFFINITY_UNSPECIFIED, NO_AFFINITY, ANTI_AFFINITY</rdfs:comment>
    <rdfs:domain rdf:resource="http://example.org/onto/class/google_gke_hub_feature_membership"/>
    <rdfs:range rdf:resource="http://www.w3.org/2001/XMLSchema#string"/>
  </owl:DatatypeProperty>
  <owl:DatatypeProperty rdf:about="http://example.org/onto/prop/google_gke_hub_feature_membership_replica_count">
    <rdfs:label>replica_count</rdfs:label>
    <rdfs:comment>Pod replica count.</rdfs:comment>
    <rdfs:domain rdf:resource="http://example.org/onto/class/google_gke_hub_feature_membership"/>
    <rdfs:range rdf:resource="http://www.w3.org/2001/XMLSchema#string"/>
  </owl:DatatypeProperty>
  <owl:DatatypeProperty rdf:about="http://example.org/onto/prop/google_gke_hub_feature_membership_cpu">
    <rdfs:label>cpu</rdfs:label>
    <rdfs:comment>CPU requirement expressed in Kubernetes resource units.</rdfs:comment>
    <rdfs:domain rdf:resource="http://example.org/onto/class/google_gke_hub_feature_membership"/>
    <rdfs:range rdf:resource="http://www.w3.org/2001/XMLSchema#string"/>
  </owl:DatatypeProperty>
  <owl:DatatypeProperty rdf:about="http://example.org/onto/prop/google_gke_hub_feature_membership_memory">
    <rdfs:label>memory</rdfs:label>
    <rdfs:comment>Memory requirement expressed in Kubernetes resource units.</rdfs:comment>
    <rdfs:domain rdf:resource="http://example.org/onto/class/google_gke_hub_feature_membership"/>
    <rdfs:range rdf:resource="http://www.w3.org/2001/XMLSchema#string"/>
  </owl:DatatypeProperty>
  <owl:DatatypeProperty rdf:about="http://example.org/onto/prop/google_gke_hub_feature_membership_cpu">
    <rdfs:label>cpu</rdfs:label>
    <rdfs:comment>CPU requirement expressed in Kubernetes resource units.</rdfs:comment>
    <rdfs:domain rdf:resource="http://example.org/onto/class/google_gke_hub_feature_membership"/>
    <rdfs:range rdf:resource="http://www.w3.org/2001/XMLSchema#string"/>
  </owl:DatatypeProperty>
  <owl:DatatypeProperty rdf:about="http://example.org/onto/prop/google_gke_hub_feature_membership_memory">
    <rdfs:label>memory</rdfs:label>
    <rdfs:comment>Memory requirement expressed in Kubernetes resource units.</rdfs:comment>
    <rdfs:domain rdf:resource="http://example.org/onto/class/google_gke_hub_feature_membership"/>
    <rdfs:range rdf:resource="http://www.w3.org/2001/XMLSchema#string"/>
  </owl:DatatypeProperty>
  <owl:DatatypeProperty rdf:about="http://example.org/onto/prop/google_gke_hub_feature_membership_effect">
    <rdfs:label>effect</rdfs:label>
    <rdfs:comment>Matches a taint effect.</rdfs:comment>
    <rdfs:domain rdf:resource="http://example.org/onto/class/google_gke_hub_feature_membership"/>
    <rdfs:range rdf:resource="http://www.w3.org/2001/XMLSchema#string"/>
  </owl:DatatypeProperty>
  <owl:DatatypeProperty rdf:about="http://example.org/onto/prop/google_gke_hub_feature_membership_key">
    <rdfs:label>key</rdfs:label>
    <rdfs:comment>Matches a taint key (not necessarily unique).</rdfs:comment>
    <rdfs:domain rdf:resource="http://example.org/onto/class/google_gke_hub_feature_membership"/>
    <rdfs:range rdf:resource="http://www.w3.org/2001/XMLSchema#string"/>
  </owl:DatatypeProperty>
  <owl:DatatypeProperty rdf:about="http://example.org/onto/prop/google_gke_hub_feature_membership_operator">
    <rdfs:label>operator</rdfs:label>
    <rdfs:comment>Matches a taint operator.</rdfs:comment>
    <rdfs:domain rdf:resource="http://example.org/onto/class/google_gke_hub_feature_membership"/>
    <rdfs:range rdf:resource="http://www.w3.org/2001/XMLSchema#string"/>
  </owl:DatatypeProperty>
  <owl:DatatypeProperty rdf:about="http://example.org/onto/prop/google_gke_hub_feature_membership_value">
    <rdfs:label>value</rdfs:label>
    <rdfs:comment>Matches a taint value.</rdfs:comment>
    <rdfs:domain rdf:resource="http://example.org/onto/class/google_gke_hub_feature_membership"/>
    <rdfs:range rdf:resource="http://www.w3.org/2001/XMLSchema#string"/>
  </owl:DatatypeProperty>
  <owl:DatatypeProperty rdf:about="http://example.org/onto/prop/google_gke_hub_feature_membership_backends">
    <rdfs:label>backends</rdfs:label>
    <rdfs:comment>Specifies the list of backends Policy Controller will export to. Specifying an empty value `[]` disables metrics export.</rdfs:comment>
    <rdfs:domain rdf:resource="http://example.org/onto/class/google_gke_hub_feature_membership"/>
    <rdfs:range rdf:resource="http://www.w3.org/2001/XMLSchema#string"/>
  </owl:DatatypeProperty>
  <owl:DatatypeProperty rdf:about="http://example.org/onto/prop/google_gke_hub_feature_membership_bundle_name">
    <rdfs:label>bundle_name</rdfs:label>
    <rdfs:comment>The name for the key in the map for which this object is mapped to in the API</rdfs:comment>
    <rdfs:domain rdf:resource="http://example.org/onto/class/google_gke_hub_feature_membership"/>
    <rdfs:range rdf:resource="http://www.w3.org/2001/XMLSchema#string"/>
  </owl:DatatypeProperty>
  <owl:DatatypeProperty rdf:about="http://example.org/onto/prop/google_gke_hub_feature_membership_exempted_namespaces">
    <rdfs:label>exempted_namespaces</rdfs:label>
    <rdfs:comment>The set of namespaces to be exempted from the bundle.</rdfs:comment>
    <rdfs:domain rdf:resource="http://example.org/onto/class/google_gke_hub_feature_membership"/>
    <rdfs:range rdf:resource="http://www.w3.org/2001/XMLSchema#string"/>
  </owl:DatatypeProperty>
  <owl:DatatypeProperty rdf:about="http://example.org/onto/prop/google_gke_hub_feature_membership_installation">
    <rdfs:label>installation</rdfs:label>
    <rdfs:comment>Configures the manner in which the template library is installed on the cluster. Possible values: INSTALLATION_UNSPECIFIED, NOT_INSTALLED, ALL</rdfs:comment>
    <rdfs:domain rdf:resource="http://example.org/onto/class/google_gke_hub_feature_membership"/>
    <rdfs:range rdf:resource="http://www.w3.org/2001/XMLSchema#string"/>
  </owl:DatatypeProperty>
  <owl:DatatypeProperty rdf:about="http://example.org/onto/prop/google_gke_hub_feature_membership_create">
    <rdfs:label>create</rdfs:label>
    <rdfs:domain rdf:resource="http://example.org/onto/class/google_gke_hub_feature_membership"/>
    <rdfs:range rdf:resource="http://www.w3.org/2001/XMLSchema#string"/>
  </owl:DatatypeProperty>
  <owl:DatatypeProperty rdf:about="http://example.org/onto/prop/google_gke_hub_feature_membership_delete">
    <rdfs:label>delete</rdfs:label>
    <rdfs:domain rdf:resource="http://example.org/onto/class/google_gke_hub_feature_membership"/>
    <rdfs:range rdf:resource="http://www.w3.org/2001/XMLSchema#string"/>
  </owl:DatatypeProperty>
  <owl:DatatypeProperty rdf:about="http://example.org/onto/prop/google_gke_hub_feature_membership_update">
    <rdfs:label>update</rdfs:label>
    <rdfs:domain rdf:resource="http://example.org/onto/class/google_gke_hub_feature_membership"/>
    <rdfs:range rdf:resource="http://www.w3.org/2001/XMLSchema#string"/>
  </owl:DatatypeProperty>
</rdf:RDF>
