<?xml version="1.0" encoding="UTF-8"?>
<rdf:RDF
  xmlns:rdf="http://www.w3.org/1999/02/22-rdf-syntax-ns#"
  xmlns:rdfs="http://www.w3.org/2000/01/rdf-schema#"
  xmlns:owl="http://www.w3.org/2002/07/owl#"
  xmlns:xsd="http://www.w3.org/2001/XMLSchema#"
  xml:base="http://example.org/onto/">
  <owl:Class rdf:about="http://example.org/onto/class/google_network_services_tcp_route">
    <rdfs:label>google_network_services_tcp_route</rdfs:label>
    <rdfs:comment>#
#     ***     AUTO GENERATED CODE    ***    Type: MMv1     ***
#
# ----------------------------------------------------------------------------
#
#     This code is generated by Magic Modules using the following:
#
#     Configuration: https:#github.com/GoogleCloudPlatform/magic-modules/tree/main/mmv1/products/networkservices/TcpRoute.yaml
#     Template:      https:#github.com/GoogleCloudPlatform/magic-modules/tree/main/mmv1/templates/terraform/resource.html.markdown.tmpl
#
#     DO NOT EDIT this file directly. Any changes made to this file will be
#     overwritten during the next generation cycle.
#
# ----------------------------------------------------------------------------
subcategory: "Network Services"
description: |-
  TcpRoute is the resource defining how TCP traffic should be routed by a Mesh/Gateway resource.
---</rdfs:comment>
  </owl:Class>
  <owl:DatatypeProperty rdf:about="http://example.org/onto/prop/google_network_services_tcp_route_create_time">
    <rdfs:label>create_time</rdfs:label>
    <rdfs:comment>Time the TcpRoute was created in UTC.</rdfs:comment>
    <rdfs:domain rdf:resource="http://example.org/onto/class/google_network_services_tcp_route"/>
    <rdfs:range rdf:resource="http://www.w3.org/2001/XMLSchema#string"/>
  </owl:DatatypeProperty>
  <owl:DatatypeProperty rdf:about="http://example.org/onto/prop/google_network_services_tcp_route_description">
    <rdfs:label>description</rdfs:label>
    <rdfs:comment>A free-text description of the resource. Max length 1024 characters.</rdfs:comment>
    <rdfs:domain rdf:resource="http://example.org/onto/class/google_network_services_tcp_route"/>
    <rdfs:range rdf:resource="http://www.w3.org/2001/XMLSchema#string"/>
  </owl:DatatypeProperty>
  <owl:DatatypeProperty rdf:about="http://example.org/onto/prop/google_network_services_tcp_route_effective_labels">
    <rdfs:label>effective_labels</rdfs:label>
    <rdfs:comment>All of labels (key/value pairs) present on the resource in GCP, including the labels configured through Terraform, other clients and services.</rdfs:comment>
    <rdfs:domain rdf:resource="http://example.org/onto/class/google_network_services_tcp_route"/>
    <rdfs:range rdf:resource="http://www.w3.org/2001/XMLSchema#string"/>
  </owl:DatatypeProperty>
  <owl:DatatypeProperty rdf:about="http://example.org/onto/prop/google_network_services_tcp_route_gateways">
    <rdfs:label>gateways</rdfs:label>
    <rdfs:comment>Gateways defines a list of gateways this TcpRoute is attached to, as one of the routing rules to route the requests served by the gateway.
Each gateway reference should match the pattern: projects/*/locations/global/gateways/<gateway_name></rdfs:comment>
    <rdfs:domain rdf:resource="http://example.org/onto/class/google_network_services_tcp_route"/>
    <rdfs:range rdf:resource="http://www.w3.org/2001/XMLSchema#string"/>
  </owl:DatatypeProperty>
  <owl:DatatypeProperty rdf:about="http://example.org/onto/prop/google_network_services_tcp_route_id">
    <rdfs:label>id</rdfs:label>
    <rdfs:domain rdf:resource="http://example.org/onto/class/google_network_services_tcp_route"/>
    <rdfs:range rdf:resource="http://www.w3.org/2001/XMLSchema#string"/>
  </owl:DatatypeProperty>
  <owl:DatatypeProperty rdf:about="http://example.org/onto/prop/google_network_services_tcp_route_labels">
    <rdfs:label>labels</rdfs:label>
    <rdfs:comment>Set of label tags associated with the TcpRoute resource.

**Note**: This field is non-authoritative, and will only manage the labels present in your configuration.
Please refer to the field 'effective_labels' for all of the labels present on the resource.</rdfs:comment>
    <rdfs:domain rdf:resource="http://example.org/onto/class/google_network_services_tcp_route"/>
    <rdfs:range rdf:resource="http://www.w3.org/2001/XMLSchema#string"/>
  </owl:DatatypeProperty>
  <owl:DatatypeProperty rdf:about="http://example.org/onto/prop/google_network_services_tcp_route_meshes">
    <rdfs:label>meshes</rdfs:label>
    <rdfs:comment>Meshes defines a list of meshes this TcpRoute is attached to, as one of the routing rules to route the requests served by the mesh.
Each mesh reference should match the pattern: projects/*/locations/global/meshes/<mesh_name>
The attached Mesh should be of a type SIDECAR</rdfs:comment>
    <rdfs:domain rdf:resource="http://example.org/onto/class/google_network_services_tcp_route"/>
    <rdfs:range rdf:resource="http://www.w3.org/2001/XMLSchema#string"/>
  </owl:DatatypeProperty>
  <owl:DatatypeProperty rdf:about="http://example.org/onto/prop/google_network_services_tcp_route_name">
    <rdfs:label>name</rdfs:label>
    <rdfs:comment>Name of the TcpRoute resource.</rdfs:comment>
    <rdfs:domain rdf:resource="http://example.org/onto/class/google_network_services_tcp_route"/>
    <rdfs:range rdf:resource="http://www.w3.org/2001/XMLSchema#string"/>
  </owl:DatatypeProperty>
  <owl:DatatypeProperty rdf:about="http://example.org/onto/prop/google_network_services_tcp_route_project">
    <rdfs:label>project</rdfs:label>
    <rdfs:domain rdf:resource="http://example.org/onto/class/google_network_services_tcp_route"/>
    <rdfs:range rdf:resource="http://www.w3.org/2001/XMLSchema#string"/>
  </owl:DatatypeProperty>
  <owl:DatatypeProperty rdf:about="http://example.org/onto/prop/google_network_services_tcp_route_self_link">
    <rdfs:label>self_link</rdfs:label>
    <rdfs:comment>Server-defined URL of this resource.</rdfs:comment>
    <rdfs:domain rdf:resource="http://example.org/onto/class/google_network_services_tcp_route"/>
    <rdfs:range rdf:resource="http://www.w3.org/2001/XMLSchema#string"/>
  </owl:DatatypeProperty>
  <owl:DatatypeProperty rdf:about="http://example.org/onto/prop/google_network_services_tcp_route_terraform_labels">
    <rdfs:label>terraform_labels</rdfs:label>
    <rdfs:comment>The combination of labels configured directly on the resource
 and default labels configured on the provider.</rdfs:comment>
    <rdfs:domain rdf:resource="http://example.org/onto/class/google_network_services_tcp_route"/>
    <rdfs:range rdf:resource="http://www.w3.org/2001/XMLSchema#string"/>
  </owl:DatatypeProperty>
  <owl:DatatypeProperty rdf:about="http://example.org/onto/prop/google_network_services_tcp_route_update_time">
    <rdfs:label>update_time</rdfs:label>
    <rdfs:comment>Time the TcpRoute was updated in UTC.</rdfs:comment>
    <rdfs:domain rdf:resource="http://example.org/onto/class/google_network_services_tcp_route"/>
    <rdfs:range rdf:resource="http://www.w3.org/2001/XMLSchema#string"/>
  </owl:DatatypeProperty>
  <owl:DatatypeProperty rdf:about="http://example.org/onto/prop/google_network_services_tcp_route_idle_timeout">
    <rdfs:label>idle_timeout</rdfs:label>
    <rdfs:comment>Specifies the idle timeout for the selected route. The idle timeout is defined as the period in which there are no bytes sent or received on either the upstream or downstream connection. If not set, the default idle timeout is 30 seconds. If set to 0s, the timeout will be disabled.

A duration in seconds with up to nine fractional digits, ending with 's'. Example: "3.5s".</rdfs:comment>
    <rdfs:domain rdf:resource="http://example.org/onto/class/google_network_services_tcp_route"/>
    <rdfs:range rdf:resource="http://www.w3.org/2001/XMLSchema#string"/>
  </owl:DatatypeProperty>
  <owl:DatatypeProperty rdf:about="http://example.org/onto/prop/google_network_services_tcp_route_original_destination">
    <rdfs:label>original_destination</rdfs:label>
    <rdfs:comment>If true, Router will use the destination IP and port of the original connection as the destination of the request.</rdfs:comment>
    <rdfs:domain rdf:resource="http://example.org/onto/class/google_network_services_tcp_route"/>
    <rdfs:range rdf:resource="http://www.w3.org/2001/XMLSchema#string"/>
  </owl:DatatypeProperty>
  <owl:DatatypeProperty rdf:about="http://example.org/onto/prop/google_network_services_tcp_route_service_name">
    <rdfs:label>service_name</rdfs:label>
    <rdfs:comment>The URL of a BackendService to route traffic to.</rdfs:comment>
    <rdfs:domain rdf:resource="http://example.org/onto/class/google_network_services_tcp_route"/>
    <rdfs:range rdf:resource="http://www.w3.org/2001/XMLSchema#string"/>
  </owl:DatatypeProperty>
  <owl:DatatypeProperty rdf:about="http://example.org/onto/prop/google_network_services_tcp_route_weight">
    <rdfs:label>weight</rdfs:label>
    <rdfs:comment>Specifies the proportion of requests forwarded to the backend referenced by the serviceName field. This is computed as: weight/Sum(weights in this destination list). For non-zero values, there may be some epsilon from the exact proportion defined here depending on the precision an implementation supports.
If only one serviceName is specified and it has a weight greater than 0, 100% of the traffic is forwarded to that backend.
If weights are specified for any one service name, they need to be specified for all of them.
If weights are unspecified for all services, then, traffic is distributed in equal proportions to all of them.</rdfs:comment>
    <rdfs:domain rdf:resource="http://example.org/onto/class/google_network_services_tcp_route"/>
    <rdfs:range rdf:resource="http://www.w3.org/2001/XMLSchema#string"/>
  </owl:DatatypeProperty>
  <owl:DatatypeProperty rdf:about="http://example.org/onto/prop/google_network_services_tcp_route_address">
    <rdfs:label>address</rdfs:label>
    <rdfs:comment>Must be specified in the CIDR range format. A CIDR range consists of an IP Address and a prefix length to construct the subnet mask.
By default, the prefix length is 32 (i.e. matches a single IP address). Only IPV4 addresses are supported. Examples: "10.0.0.1" - matches against this exact IP address. "10.0.0.0/8" - matches against any IP address within the 10.0.0.0 subnet and 255.255.255.0 mask. "0.0.0.0/0" - matches against any IP address'.</rdfs:comment>
    <rdfs:domain rdf:resource="http://example.org/onto/class/google_network_services_tcp_route"/>
    <rdfs:range rdf:resource="http://www.w3.org/2001/XMLSchema#string"/>
  </owl:DatatypeProperty>
  <owl:DatatypeProperty rdf:about="http://example.org/onto/prop/google_network_services_tcp_route_port">
    <rdfs:label>port</rdfs:label>
    <rdfs:comment>Specifies the destination port to match against.</rdfs:comment>
    <rdfs:domain rdf:resource="http://example.org/onto/class/google_network_services_tcp_route"/>
    <rdfs:range rdf:resource="http://www.w3.org/2001/XMLSchema#string"/>
  </owl:DatatypeProperty>
  <owl:DatatypeProperty rdf:about="http://example.org/onto/prop/google_network_services_tcp_route_create">
    <rdfs:label>create</rdfs:label>
    <rdfs:domain rdf:resource="http://example.org/onto/class/google_network_services_tcp_route"/>
    <rdfs:range rdf:resource="http://www.w3.org/2001/XMLSchema#string"/>
  </owl:DatatypeProperty>
  <owl:DatatypeProperty rdf:about="http://example.org/onto/prop/google_network_services_tcp_route_delete">
    <rdfs:label>delete</rdfs:label>
    <rdfs:domain rdf:resource="http://example.org/onto/class/google_network_services_tcp_route"/>
    <rdfs:range rdf:resource="http://www.w3.org/2001/XMLSchema#string"/>
  </owl:DatatypeProperty>
  <owl:DatatypeProperty rdf:about="http://example.org/onto/prop/google_network_services_tcp_route_update">
    <rdfs:label>update</rdfs:label>
    <rdfs:domain rdf:resource="http://example.org/onto/class/google_network_services_tcp_route"/>
    <rdfs:range rdf:resource="http://www.w3.org/2001/XMLSchema#string"/>
  </owl:DatatypeProperty>
</rdf:RDF>
