<?xml version="1.0" encoding="UTF-8"?>
<rdf:RDF
  xmlns:rdf="http://www.w3.org/1999/02/22-rdf-syntax-ns#"
  xmlns:rdfs="http://www.w3.org/2000/01/rdf-schema#"
  xmlns:owl="http://www.w3.org/2002/07/owl#"
  xmlns:xsd="http://www.w3.org/2001/XMLSchema#"
  xml:base="http://example.org/onto/">
  <owl:Class rdf:about="http://example.org/onto/class/google_cloud_asset_folder_feed">
    <rdfs:label>google_cloud_asset_folder_feed</rdfs:label>
    <rdfs:comment>#
#     ***     AUTO GENERATED CODE    ***    Type: MMv1     ***
#
# ----------------------------------------------------------------------------
#
#     This code is generated by Magic Modules using the following:
#
#     Configuration: https:#github.com/GoogleCloudPlatform/magic-modules/tree/main/mmv1/products/cloudasset/FolderFeed.yaml
#     Template:      https:#github.com/GoogleCloudPlatform/magic-modules/tree/main/mmv1/templates/terraform/resource.html.markdown.tmpl
#
#     DO NOT EDIT this file directly. Any changes made to this file will be
#     overwritten during the next generation cycle.
#
# ----------------------------------------------------------------------------
subcategory: "Cloud Asset Inventory"
description: |-
  Describes a Cloud Asset Inventory feed used to to listen to asset updates.
---</rdfs:comment>
  </owl:Class>
  <owl:DatatypeProperty rdf:about="http://example.org/onto/prop/google_cloud_asset_folder_feed_asset_names">
    <rdfs:label>asset_names</rdfs:label>
    <rdfs:comment>A list of the full names of the assets to receive updates. You must specify either or both of
assetNames and assetTypes. Only asset updates matching specified assetNames and assetTypes are
exported to the feed. For example: //compute.googleapis.com/projects/my_project_123/zones/zone1/instances/instance1.
See https://cloud.google.com/apis/design/resourceNames#fullResourceName for more info.</rdfs:comment>
    <rdfs:domain rdf:resource="http://example.org/onto/class/google_cloud_asset_folder_feed"/>
    <rdfs:range rdf:resource="http://www.w3.org/2001/XMLSchema#string"/>
  </owl:DatatypeProperty>
  <owl:DatatypeProperty rdf:about="http://example.org/onto/prop/google_cloud_asset_folder_feed_asset_types">
    <rdfs:label>asset_types</rdfs:label>
    <rdfs:comment>A list of types of the assets to receive updates. You must specify either or both of assetNames
and assetTypes. Only asset updates matching specified assetNames and assetTypes are exported to
the feed. For example: "compute.googleapis.com/Disk"
See https://cloud.google.com/asset-inventory/docs/supported-asset-types for a list of all
supported asset types.</rdfs:comment>
    <rdfs:domain rdf:resource="http://example.org/onto/class/google_cloud_asset_folder_feed"/>
    <rdfs:range rdf:resource="http://www.w3.org/2001/XMLSchema#string"/>
  </owl:DatatypeProperty>
  <owl:DatatypeProperty rdf:about="http://example.org/onto/prop/google_cloud_asset_folder_feed_billing_project">
    <rdfs:label>billing_project</rdfs:label>
    <rdfs:comment>The project whose identity will be used when sending messages to the
destination pubsub topic. It also specifies the project for API
enablement check, quota, and billing.</rdfs:comment>
    <rdfs:domain rdf:resource="http://example.org/onto/class/google_cloud_asset_folder_feed"/>
    <rdfs:range rdf:resource="http://www.w3.org/2001/XMLSchema#string"/>
  </owl:DatatypeProperty>
  <owl:DatatypeProperty rdf:about="http://example.org/onto/prop/google_cloud_asset_folder_feed_content_type">
    <rdfs:label>content_type</rdfs:label>
    <rdfs:comment>Asset content type. If not specified, no content but the asset name and type will be returned. Possible values: ["CONTENT_TYPE_UNSPECIFIED", "RESOURCE", "IAM_POLICY", "ORG_POLICY", "OS_INVENTORY", "ACCESS_POLICY"]</rdfs:comment>
    <rdfs:domain rdf:resource="http://example.org/onto/class/google_cloud_asset_folder_feed"/>
    <rdfs:range rdf:resource="http://www.w3.org/2001/XMLSchema#string"/>
  </owl:DatatypeProperty>
  <owl:DatatypeProperty rdf:about="http://example.org/onto/prop/google_cloud_asset_folder_feed_feed_id">
    <rdfs:label>feed_id</rdfs:label>
    <rdfs:comment>This is the client-assigned asset feed identifier and it needs to be unique under a specific parent.</rdfs:comment>
    <rdfs:domain rdf:resource="http://example.org/onto/class/google_cloud_asset_folder_feed"/>
    <rdfs:range rdf:resource="http://www.w3.org/2001/XMLSchema#string"/>
  </owl:DatatypeProperty>
  <owl:DatatypeProperty rdf:about="http://example.org/onto/prop/google_cloud_asset_folder_feed_folder">
    <rdfs:label>folder</rdfs:label>
    <rdfs:comment>The folder this feed should be created in.</rdfs:comment>
    <rdfs:domain rdf:resource="http://example.org/onto/class/google_cloud_asset_folder_feed"/>
    <rdfs:range rdf:resource="http://www.w3.org/2001/XMLSchema#string"/>
  </owl:DatatypeProperty>
  <owl:DatatypeProperty rdf:about="http://example.org/onto/prop/google_cloud_asset_folder_feed_folder_id">
    <rdfs:label>folder_id</rdfs:label>
    <rdfs:comment>The ID of the folder where this feed has been created. Both [FOLDER_NUMBER]
and folders/[FOLDER_NUMBER] are accepted.</rdfs:comment>
    <rdfs:domain rdf:resource="http://example.org/onto/class/google_cloud_asset_folder_feed"/>
    <rdfs:range rdf:resource="http://www.w3.org/2001/XMLSchema#string"/>
  </owl:DatatypeProperty>
  <owl:DatatypeProperty rdf:about="http://example.org/onto/prop/google_cloud_asset_folder_feed_id">
    <rdfs:label>id</rdfs:label>
    <rdfs:domain rdf:resource="http://example.org/onto/class/google_cloud_asset_folder_feed"/>
    <rdfs:range rdf:resource="http://www.w3.org/2001/XMLSchema#string"/>
  </owl:DatatypeProperty>
  <owl:DatatypeProperty rdf:about="http://example.org/onto/prop/google_cloud_asset_folder_feed_name">
    <rdfs:label>name</rdfs:label>
    <rdfs:comment>The format will be folders/{folder_number}/feeds/{client-assigned_feed_identifier}.</rdfs:comment>
    <rdfs:domain rdf:resource="http://example.org/onto/class/google_cloud_asset_folder_feed"/>
    <rdfs:range rdf:resource="http://www.w3.org/2001/XMLSchema#string"/>
  </owl:DatatypeProperty>
  <owl:DatatypeProperty rdf:about="http://example.org/onto/prop/google_cloud_asset_folder_feed_description">
    <rdfs:label>description</rdfs:label>
    <rdfs:comment>Description of the expression. This is a longer text which describes the expression,
e.g. when hovered over it in a UI.</rdfs:comment>
    <rdfs:domain rdf:resource="http://example.org/onto/class/google_cloud_asset_folder_feed"/>
    <rdfs:range rdf:resource="http://www.w3.org/2001/XMLSchema#string"/>
  </owl:DatatypeProperty>
  <owl:DatatypeProperty rdf:about="http://example.org/onto/prop/google_cloud_asset_folder_feed_expression">
    <rdfs:label>expression</rdfs:label>
    <rdfs:comment>Textual representation of an expression in Common Expression Language syntax.</rdfs:comment>
    <rdfs:domain rdf:resource="http://example.org/onto/class/google_cloud_asset_folder_feed"/>
    <rdfs:range rdf:resource="http://www.w3.org/2001/XMLSchema#string"/>
  </owl:DatatypeProperty>
  <owl:DatatypeProperty rdf:about="http://example.org/onto/prop/google_cloud_asset_folder_feed_location">
    <rdfs:label>location</rdfs:label>
    <rdfs:comment>String indicating the location of the expression for error reporting, e.g. a file
name and a position in the file.</rdfs:comment>
    <rdfs:domain rdf:resource="http://example.org/onto/class/google_cloud_asset_folder_feed"/>
    <rdfs:range rdf:resource="http://www.w3.org/2001/XMLSchema#string"/>
  </owl:DatatypeProperty>
  <owl:DatatypeProperty rdf:about="http://example.org/onto/prop/google_cloud_asset_folder_feed_title">
    <rdfs:label>title</rdfs:label>
    <rdfs:comment>Title for the expression, i.e. a short string describing its purpose.
This can be used e.g. in UIs which allow to enter the expression.</rdfs:comment>
    <rdfs:domain rdf:resource="http://example.org/onto/class/google_cloud_asset_folder_feed"/>
    <rdfs:range rdf:resource="http://www.w3.org/2001/XMLSchema#string"/>
  </owl:DatatypeProperty>
  <owl:DatatypeProperty rdf:about="http://example.org/onto/prop/google_cloud_asset_folder_feed_topic">
    <rdfs:label>topic</rdfs:label>
    <rdfs:comment>Destination on Cloud Pubsub topic.</rdfs:comment>
    <rdfs:domain rdf:resource="http://example.org/onto/class/google_cloud_asset_folder_feed"/>
    <rdfs:range rdf:resource="http://www.w3.org/2001/XMLSchema#string"/>
  </owl:DatatypeProperty>
  <owl:DatatypeProperty rdf:about="http://example.org/onto/prop/google_cloud_asset_folder_feed_create">
    <rdfs:label>create</rdfs:label>
    <rdfs:domain rdf:resource="http://example.org/onto/class/google_cloud_asset_folder_feed"/>
    <rdfs:range rdf:resource="http://www.w3.org/2001/XMLSchema#string"/>
  </owl:DatatypeProperty>
  <owl:DatatypeProperty rdf:about="http://example.org/onto/prop/google_cloud_asset_folder_feed_delete">
    <rdfs:label>delete</rdfs:label>
    <rdfs:domain rdf:resource="http://example.org/onto/class/google_cloud_asset_folder_feed"/>
    <rdfs:range rdf:resource="http://www.w3.org/2001/XMLSchema#string"/>
  </owl:DatatypeProperty>
  <owl:DatatypeProperty rdf:about="http://example.org/onto/prop/google_cloud_asset_folder_feed_update">
    <rdfs:label>update</rdfs:label>
    <rdfs:domain rdf:resource="http://example.org/onto/class/google_cloud_asset_folder_feed"/>
    <rdfs:range rdf:resource="http://www.w3.org/2001/XMLSchema#string"/>
  </owl:DatatypeProperty>
</rdf:RDF>
