<?xml version="1.0" encoding="UTF-8"?>
<rdf:RDF
  xmlns:rdf="http://www.w3.org/1999/02/22-rdf-syntax-ns#"
  xmlns:rdfs="http://www.w3.org/2000/01/rdf-schema#"
  xmlns:owl="http://www.w3.org/2002/07/owl#"
  xmlns:xsd="http://www.w3.org/2001/XMLSchema#"
  xml:base="http://example.org/onto/">
  <owl:Class rdf:about="http://example.org/onto/class/google_compute_router_nat">
    <rdfs:label>google_compute_router_nat</rdfs:label>
    <rdfs:comment>#
#     ***     AUTO GENERATED CODE    ***    Type: MMv1     ***
#
# ----------------------------------------------------------------------------
#
#     This code is generated by Magic Modules using the following:
#
#     Configuration: https:#github.com/GoogleCloudPlatform/magic-modules/tree/main/mmv1/products/compute/RouterNat.yaml
#     Template:      https:#github.com/GoogleCloudPlatform/magic-modules/tree/main/mmv1/templates/terraform/resource.html.markdown.tmpl
#
#     DO NOT EDIT this file directly. Any changes made to this file will be
#     overwritten during the next generation cycle.
#
# ----------------------------------------------------------------------------
subcategory: "Compute Engine"
description: |-
  A NAT service created in a router.
---</rdfs:comment>
  </owl:Class>
  <owl:DatatypeProperty rdf:about="http://example.org/onto/prop/google_compute_router_nat_auto_network_tier">
    <rdfs:label>auto_network_tier</rdfs:label>
    <rdfs:comment>The network tier to use when automatically reserving NAT IP addresses.
Must be one of: PREMIUM, STANDARD. If not specified, then the current
project-level default tier is used. Possible values: ["PREMIUM", "STANDARD"]</rdfs:comment>
    <rdfs:domain rdf:resource="http://example.org/onto/class/google_compute_router_nat"/>
    <rdfs:range rdf:resource="http://www.w3.org/2001/XMLSchema#string"/>
  </owl:DatatypeProperty>
  <owl:DatatypeProperty rdf:about="http://example.org/onto/prop/google_compute_router_nat_drain_nat_ips">
    <rdfs:label>drain_nat_ips</rdfs:label>
    <rdfs:comment>A list of URLs of the IP resources to be drained. These IPs must be
valid static external IPs that have been assigned to the NAT.</rdfs:comment>
    <rdfs:domain rdf:resource="http://example.org/onto/class/google_compute_router_nat"/>
    <rdfs:range rdf:resource="http://www.w3.org/2001/XMLSchema#string"/>
  </owl:DatatypeProperty>
  <owl:DatatypeProperty rdf:about="http://example.org/onto/prop/google_compute_router_nat_enable_dynamic_port_allocation">
    <rdfs:label>enable_dynamic_port_allocation</rdfs:label>
    <rdfs:comment>Enable Dynamic Port Allocation.
If minPortsPerVm is set, minPortsPerVm must be set to a power of two greater than or equal to 32.
If minPortsPerVm is not set, a minimum of 32 ports will be allocated to a VM from this NAT config.
If maxPortsPerVm is set, maxPortsPerVm must be set to a power of two greater than minPortsPerVm.
If maxPortsPerVm is not set, a maximum of 65536 ports will be allocated to a VM from this NAT config.

Mutually exclusive with enableEndpointIndependentMapping.</rdfs:comment>
    <rdfs:domain rdf:resource="http://example.org/onto/class/google_compute_router_nat"/>
    <rdfs:range rdf:resource="http://www.w3.org/2001/XMLSchema#string"/>
  </owl:DatatypeProperty>
  <owl:DatatypeProperty rdf:about="http://example.org/onto/prop/google_compute_router_nat_enable_endpoint_independent_mapping">
    <rdfs:label>enable_endpoint_independent_mapping</rdfs:label>
    <rdfs:comment>Enable endpoint independent mapping.
For more information see the [official documentation](https://cloud.google.com/nat/docs/overview#specs-rfcs).</rdfs:comment>
    <rdfs:domain rdf:resource="http://example.org/onto/class/google_compute_router_nat"/>
    <rdfs:range rdf:resource="http://www.w3.org/2001/XMLSchema#string"/>
  </owl:DatatypeProperty>
  <owl:DatatypeProperty rdf:about="http://example.org/onto/prop/google_compute_router_nat_endpoint_types">
    <rdfs:label>endpoint_types</rdfs:label>
    <rdfs:comment>Specifies the endpoint Types supported by the NAT Gateway.
Supported values include:
      'ENDPOINT_TYPE_VM', 'ENDPOINT_TYPE_SWG',
      'ENDPOINT_TYPE_MANAGED_PROXY_LB'.</rdfs:comment>
    <rdfs:domain rdf:resource="http://example.org/onto/class/google_compute_router_nat"/>
    <rdfs:range rdf:resource="http://www.w3.org/2001/XMLSchema#string"/>
  </owl:DatatypeProperty>
  <owl:DatatypeProperty rdf:about="http://example.org/onto/prop/google_compute_router_nat_icmp_idle_timeout_sec">
    <rdfs:label>icmp_idle_timeout_sec</rdfs:label>
    <rdfs:comment>Timeout (in seconds) for ICMP connections. Defaults to 30s if not set.</rdfs:comment>
    <rdfs:domain rdf:resource="http://example.org/onto/class/google_compute_router_nat"/>
    <rdfs:range rdf:resource="http://www.w3.org/2001/XMLSchema#string"/>
  </owl:DatatypeProperty>
  <owl:DatatypeProperty rdf:about="http://example.org/onto/prop/google_compute_router_nat_id">
    <rdfs:label>id</rdfs:label>
    <rdfs:domain rdf:resource="http://example.org/onto/class/google_compute_router_nat"/>
    <rdfs:range rdf:resource="http://www.w3.org/2001/XMLSchema#string"/>
  </owl:DatatypeProperty>
  <owl:DatatypeProperty rdf:about="http://example.org/onto/prop/google_compute_router_nat_initial_nat_ips">
    <rdfs:label>initial_nat_ips</rdfs:label>
    <rdfs:comment>Self-links of NAT IPs to be used as initial value for creation alongside a RouterNatAddress resource.
Conflicts with natIps and drainNatIps. Only valid if natIpAllocateOption is set to MANUAL_ONLY.</rdfs:comment>
    <rdfs:domain rdf:resource="http://example.org/onto/class/google_compute_router_nat"/>
    <rdfs:range rdf:resource="http://www.w3.org/2001/XMLSchema#string"/>
  </owl:DatatypeProperty>
  <owl:DatatypeProperty rdf:about="http://example.org/onto/prop/google_compute_router_nat_max_ports_per_vm">
    <rdfs:label>max_ports_per_vm</rdfs:label>
    <rdfs:comment>Maximum number of ports allocated to a VM from this NAT.
This field can only be set when enableDynamicPortAllocation is enabled.</rdfs:comment>
    <rdfs:domain rdf:resource="http://example.org/onto/class/google_compute_router_nat"/>
    <rdfs:range rdf:resource="http://www.w3.org/2001/XMLSchema#string"/>
  </owl:DatatypeProperty>
  <owl:DatatypeProperty rdf:about="http://example.org/onto/prop/google_compute_router_nat_min_ports_per_vm">
    <rdfs:label>min_ports_per_vm</rdfs:label>
    <rdfs:comment>Minimum number of ports allocated to a VM from this NAT. Defaults to 64 for static port allocation and 32 dynamic port allocation if not set.</rdfs:comment>
    <rdfs:domain rdf:resource="http://example.org/onto/class/google_compute_router_nat"/>
    <rdfs:range rdf:resource="http://www.w3.org/2001/XMLSchema#string"/>
  </owl:DatatypeProperty>
  <owl:DatatypeProperty rdf:about="http://example.org/onto/prop/google_compute_router_nat_name">
    <rdfs:label>name</rdfs:label>
    <rdfs:comment>Name of the NAT service. The name must be 1-63 characters long and
comply with RFC1035.</rdfs:comment>
    <rdfs:domain rdf:resource="http://example.org/onto/class/google_compute_router_nat"/>
    <rdfs:range rdf:resource="http://www.w3.org/2001/XMLSchema#string"/>
  </owl:DatatypeProperty>
  <owl:DatatypeProperty rdf:about="http://example.org/onto/prop/google_compute_router_nat_nat_ip_allocate_option">
    <rdfs:label>nat_ip_allocate_option</rdfs:label>
    <rdfs:comment>How external IPs should be allocated for this NAT. Valid values are
'AUTO_ONLY' for only allowing NAT IPs allocated by Google Cloud
Platform, or 'MANUAL_ONLY' for only user-allocated NAT IP addresses. Possible values: ["MANUAL_ONLY", "AUTO_ONLY"]</rdfs:comment>
    <rdfs:domain rdf:resource="http://example.org/onto/class/google_compute_router_nat"/>
    <rdfs:range rdf:resource="http://www.w3.org/2001/XMLSchema#string"/>
  </owl:DatatypeProperty>
  <owl:DatatypeProperty rdf:about="http://example.org/onto/prop/google_compute_router_nat_nat_ips">
    <rdfs:label>nat_ips</rdfs:label>
    <rdfs:comment>Self-links of NAT IPs. Only valid if natIpAllocateOption
is set to MANUAL_ONLY.
If this field is used alongside with a count created list of address resources 'google_compute_address.foobar.*.self_link',
the access level resource for the address resource must have a 'lifecycle' block with 'create_before_destroy = true' so
the number of resources can be increased/decreased without triggering the 'resourceInUseByAnotherResource' error.</rdfs:comment>
    <rdfs:domain rdf:resource="http://example.org/onto/class/google_compute_router_nat"/>
    <rdfs:range rdf:resource="http://www.w3.org/2001/XMLSchema#string"/>
  </owl:DatatypeProperty>
  <owl:DatatypeProperty rdf:about="http://example.org/onto/prop/google_compute_router_nat_project">
    <rdfs:label>project</rdfs:label>
    <rdfs:domain rdf:resource="http://example.org/onto/class/google_compute_router_nat"/>
    <rdfs:range rdf:resource="http://www.w3.org/2001/XMLSchema#string"/>
  </owl:DatatypeProperty>
  <owl:DatatypeProperty rdf:about="http://example.org/onto/prop/google_compute_router_nat_region">
    <rdfs:label>region</rdfs:label>
    <rdfs:comment>Region where the router and NAT reside.</rdfs:comment>
    <rdfs:domain rdf:resource="http://example.org/onto/class/google_compute_router_nat"/>
    <rdfs:range rdf:resource="http://www.w3.org/2001/XMLSchema#string"/>
  </owl:DatatypeProperty>
  <owl:DatatypeProperty rdf:about="http://example.org/onto/prop/google_compute_router_nat_router">
    <rdfs:label>router</rdfs:label>
    <rdfs:comment>The name of the Cloud Router in which this NAT will be configured.</rdfs:comment>
    <rdfs:domain rdf:resource="http://example.org/onto/class/google_compute_router_nat"/>
    <rdfs:range rdf:resource="http://www.w3.org/2001/XMLSchema#string"/>
  </owl:DatatypeProperty>
  <owl:DatatypeProperty rdf:about="http://example.org/onto/prop/google_compute_router_nat_source_subnetwork_ip_ranges_to_nat">
    <rdfs:label>source_subnetwork_ip_ranges_to_nat</rdfs:label>
    <rdfs:comment>How NAT should be configured per Subnetwork.
If 'ALL_SUBNETWORKS_ALL_IP_RANGES', all of the
IP ranges in every Subnetwork are allowed to Nat.
If 'ALL_SUBNETWORKS_ALL_PRIMARY_IP_RANGES', all of the primary IP
ranges in every Subnetwork are allowed to Nat.
'LIST_OF_SUBNETWORKS': A list of Subnetworks are allowed to Nat
(specified in the field subnetwork below). Note that if this field
contains ALL_SUBNETWORKS_ALL_IP_RANGES or
ALL_SUBNETWORKS_ALL_PRIMARY_IP_RANGES, then there should not be any
other RouterNat section in any Router for this network in this region. Possible values: ["ALL_SUBNETWORKS_ALL_IP_RANGES", "ALL_SUBNETWORKS_ALL_PRIMARY_IP_RANGES", "LIST_OF_SUBNETWORKS"]</rdfs:comment>
    <rdfs:domain rdf:resource="http://example.org/onto/class/google_compute_router_nat"/>
    <rdfs:range rdf:resource="http://www.w3.org/2001/XMLSchema#string"/>
  </owl:DatatypeProperty>
  <owl:DatatypeProperty rdf:about="http://example.org/onto/prop/google_compute_router_nat_source_subnetwork_ip_ranges_to_nat64">
    <rdfs:label>source_subnetwork_ip_ranges_to_nat64</rdfs:label>
    <rdfs:comment>Specify the Nat option for NAT64, which can take one of the following values:
ALL_IPV6_SUBNETWORKS: All of the IP ranges in every Subnetwork are allowed to Nat.
LIST_OF_IPV6_SUBNETWORKS: A list of Subnetworks are allowed to Nat (specified in the field nat64Subnetwork below).
Note that if this field contains NAT64_ALL_V6_SUBNETWORKS no other Router.Nat section in this region can also enable NAT64 for any Subnetworks in this network.
Other Router.Nat sections can still be present to enable NAT44 only. Possible values: ["ALL_IPV6_SUBNETWORKS", "LIST_OF_IPV6_SUBNETWORKS"]</rdfs:comment>
    <rdfs:domain rdf:resource="http://example.org/onto/class/google_compute_router_nat"/>
    <rdfs:range rdf:resource="http://www.w3.org/2001/XMLSchema#string"/>
  </owl:DatatypeProperty>
  <owl:DatatypeProperty rdf:about="http://example.org/onto/prop/google_compute_router_nat_tcp_established_idle_timeout_sec">
    <rdfs:label>tcp_established_idle_timeout_sec</rdfs:label>
    <rdfs:comment>Timeout (in seconds) for TCP established connections.
Defaults to 1200s if not set.</rdfs:comment>
    <rdfs:domain rdf:resource="http://example.org/onto/class/google_compute_router_nat"/>
    <rdfs:range rdf:resource="http://www.w3.org/2001/XMLSchema#string"/>
  </owl:DatatypeProperty>
  <owl:DatatypeProperty rdf:about="http://example.org/onto/prop/google_compute_router_nat_tcp_time_wait_timeout_sec">
    <rdfs:label>tcp_time_wait_timeout_sec</rdfs:label>
    <rdfs:comment>Timeout (in seconds) for TCP connections that are in TIME_WAIT state.
Defaults to 120s if not set.</rdfs:comment>
    <rdfs:domain rdf:resource="http://example.org/onto/class/google_compute_router_nat"/>
    <rdfs:range rdf:resource="http://www.w3.org/2001/XMLSchema#string"/>
  </owl:DatatypeProperty>
  <owl:DatatypeProperty rdf:about="http://example.org/onto/prop/google_compute_router_nat_tcp_transitory_idle_timeout_sec">
    <rdfs:label>tcp_transitory_idle_timeout_sec</rdfs:label>
    <rdfs:comment>Timeout (in seconds) for TCP transitory connections.
Defaults to 30s if not set.</rdfs:comment>
    <rdfs:domain rdf:resource="http://example.org/onto/class/google_compute_router_nat"/>
    <rdfs:range rdf:resource="http://www.w3.org/2001/XMLSchema#string"/>
  </owl:DatatypeProperty>
  <owl:DatatypeProperty rdf:about="http://example.org/onto/prop/google_compute_router_nat_type">
    <rdfs:label>type</rdfs:label>
    <rdfs:comment>Indicates whether this NAT is used for public or private IP translation.
If unspecified, it defaults to PUBLIC.
If 'PUBLIC' NAT used for public IP translation.
If 'PRIVATE' NAT used for private IP translation. Default value: "PUBLIC" Possible values: ["PUBLIC", "PRIVATE"]</rdfs:comment>
    <rdfs:domain rdf:resource="http://example.org/onto/class/google_compute_router_nat"/>
    <rdfs:range rdf:resource="http://www.w3.org/2001/XMLSchema#string"/>
  </owl:DatatypeProperty>
  <owl:DatatypeProperty rdf:about="http://example.org/onto/prop/google_compute_router_nat_udp_idle_timeout_sec">
    <rdfs:label>udp_idle_timeout_sec</rdfs:label>
    <rdfs:comment>Timeout (in seconds) for UDP connections. Defaults to 30s if not set.</rdfs:comment>
    <rdfs:domain rdf:resource="http://example.org/onto/class/google_compute_router_nat"/>
    <rdfs:range rdf:resource="http://www.w3.org/2001/XMLSchema#string"/>
  </owl:DatatypeProperty>
  <owl:DatatypeProperty rdf:about="http://example.org/onto/prop/google_compute_router_nat_enable">
    <rdfs:label>enable</rdfs:label>
    <rdfs:comment>Indicates whether or not to export logs.</rdfs:comment>
    <rdfs:domain rdf:resource="http://example.org/onto/class/google_compute_router_nat"/>
    <rdfs:range rdf:resource="http://www.w3.org/2001/XMLSchema#string"/>
  </owl:DatatypeProperty>
  <owl:DatatypeProperty rdf:about="http://example.org/onto/prop/google_compute_router_nat_filter">
    <rdfs:label>filter</rdfs:label>
    <rdfs:comment>Specifies the desired filtering of logs on this NAT. Possible values: ["ERRORS_ONLY", "TRANSLATIONS_ONLY", "ALL"]</rdfs:comment>
    <rdfs:domain rdf:resource="http://example.org/onto/class/google_compute_router_nat"/>
    <rdfs:range rdf:resource="http://www.w3.org/2001/XMLSchema#string"/>
  </owl:DatatypeProperty>
  <owl:DatatypeProperty rdf:about="http://example.org/onto/prop/google_compute_router_nat_name">
    <rdfs:label>name</rdfs:label>
    <rdfs:comment>Self-link of the subnetwork resource that will use NAT64</rdfs:comment>
    <rdfs:domain rdf:resource="http://example.org/onto/class/google_compute_router_nat"/>
    <rdfs:range rdf:resource="http://www.w3.org/2001/XMLSchema#string"/>
  </owl:DatatypeProperty>
  <owl:DatatypeProperty rdf:about="http://example.org/onto/prop/google_compute_router_nat_description">
    <rdfs:label>description</rdfs:label>
    <rdfs:comment>An optional description of this rule.</rdfs:comment>
    <rdfs:domain rdf:resource="http://example.org/onto/class/google_compute_router_nat"/>
    <rdfs:range rdf:resource="http://www.w3.org/2001/XMLSchema#string"/>
  </owl:DatatypeProperty>
  <owl:DatatypeProperty rdf:about="http://example.org/onto/prop/google_compute_router_nat_match">
    <rdfs:label>match</rdfs:label>
    <rdfs:comment>CEL expression that specifies the match condition that egress traffic from a VM is evaluated against.
If it evaluates to true, the corresponding action is enforced.

The following examples are valid match expressions for public NAT:

"inIpRange(destination.ip, '1.1.0.0/16') || inIpRange(destination.ip, '2.2.0.0/16')"

"destination.ip == '1.1.0.1' || destination.ip == '8.8.8.8'"

The following example is a valid match expression for private NAT:

"nexthop.hub == 'https://networkconnectivity.googleapis.com/v1alpha1/projects/my-project/global/hub/hub-1'"</rdfs:comment>
    <rdfs:domain rdf:resource="http://example.org/onto/class/google_compute_router_nat"/>
    <rdfs:range rdf:resource="http://www.w3.org/2001/XMLSchema#string"/>
  </owl:DatatypeProperty>
  <owl:DatatypeProperty rdf:about="http://example.org/onto/prop/google_compute_router_nat_rule_number">
    <rdfs:label>rule_number</rdfs:label>
    <rdfs:comment>An integer uniquely identifying a rule in the list.
The rule number must be a positive value between 0 and 65000, and must be unique among rules within a NAT.</rdfs:comment>
    <rdfs:domain rdf:resource="http://example.org/onto/class/google_compute_router_nat"/>
    <rdfs:range rdf:resource="http://www.w3.org/2001/XMLSchema#string"/>
  </owl:DatatypeProperty>
  <owl:DatatypeProperty rdf:about="http://example.org/onto/prop/google_compute_router_nat_source_nat_active_ips">
    <rdfs:label>source_nat_active_ips</rdfs:label>
    <rdfs:comment>A list of URLs of the IP resources used for this NAT rule.
These IP addresses must be valid static external IP addresses assigned to the project.
This field is used for public NAT.</rdfs:comment>
    <rdfs:domain rdf:resource="http://example.org/onto/class/google_compute_router_nat"/>
    <rdfs:range rdf:resource="http://www.w3.org/2001/XMLSchema#string"/>
  </owl:DatatypeProperty>
  <owl:DatatypeProperty rdf:about="http://example.org/onto/prop/google_compute_router_nat_source_nat_active_ranges">
    <rdfs:label>source_nat_active_ranges</rdfs:label>
    <rdfs:comment>A list of URLs of the subnetworks used as source ranges for this NAT Rule.
These subnetworks must have purpose set to PRIVATE_NAT.
This field is used for private NAT.</rdfs:comment>
    <rdfs:domain rdf:resource="http://example.org/onto/class/google_compute_router_nat"/>
    <rdfs:range rdf:resource="http://www.w3.org/2001/XMLSchema#string"/>
  </owl:DatatypeProperty>
  <owl:DatatypeProperty rdf:about="http://example.org/onto/prop/google_compute_router_nat_source_nat_drain_ips">
    <rdfs:label>source_nat_drain_ips</rdfs:label>
    <rdfs:comment>A list of URLs of the IP resources to be drained.
These IPs must be valid static external IPs that have been assigned to the NAT.
These IPs should be used for updating/patching a NAT rule only.
This field is used for public NAT.</rdfs:comment>
    <rdfs:domain rdf:resource="http://example.org/onto/class/google_compute_router_nat"/>
    <rdfs:range rdf:resource="http://www.w3.org/2001/XMLSchema#string"/>
  </owl:DatatypeProperty>
  <owl:DatatypeProperty rdf:about="http://example.org/onto/prop/google_compute_router_nat_source_nat_drain_ranges">
    <rdfs:label>source_nat_drain_ranges</rdfs:label>
    <rdfs:comment>A list of URLs of subnetworks representing source ranges to be drained.
This is only supported on patch/update, and these subnetworks must have previously been used as active ranges in this NAT Rule.
This field is used for private NAT.</rdfs:comment>
    <rdfs:domain rdf:resource="http://example.org/onto/class/google_compute_router_nat"/>
    <rdfs:range rdf:resource="http://www.w3.org/2001/XMLSchema#string"/>
  </owl:DatatypeProperty>
  <owl:DatatypeProperty rdf:about="http://example.org/onto/prop/google_compute_router_nat_name">
    <rdfs:label>name</rdfs:label>
    <rdfs:comment>Self-link of subnetwork to NAT</rdfs:comment>
    <rdfs:domain rdf:resource="http://example.org/onto/class/google_compute_router_nat"/>
    <rdfs:range rdf:resource="http://www.w3.org/2001/XMLSchema#string"/>
  </owl:DatatypeProperty>
  <owl:DatatypeProperty rdf:about="http://example.org/onto/prop/google_compute_router_nat_secondary_ip_range_names">
    <rdfs:label>secondary_ip_range_names</rdfs:label>
    <rdfs:comment>List of the secondary ranges of the subnetwork that are allowed
to use NAT. This can be populated only if
'LIST_OF_SECONDARY_IP_RANGES' is one of the values in
sourceIpRangesToNat</rdfs:comment>
    <rdfs:domain rdf:resource="http://example.org/onto/class/google_compute_router_nat"/>
    <rdfs:range rdf:resource="http://www.w3.org/2001/XMLSchema#string"/>
  </owl:DatatypeProperty>
  <owl:DatatypeProperty rdf:about="http://example.org/onto/prop/google_compute_router_nat_source_ip_ranges_to_nat">
    <rdfs:label>source_ip_ranges_to_nat</rdfs:label>
    <rdfs:comment>List of options for which source IPs in the subnetwork
should have NAT enabled. Supported values include:
'ALL_IP_RANGES', 'LIST_OF_SECONDARY_IP_RANGES',
'PRIMARY_IP_RANGE'.</rdfs:comment>
    <rdfs:domain rdf:resource="http://example.org/onto/class/google_compute_router_nat"/>
    <rdfs:range rdf:resource="http://www.w3.org/2001/XMLSchema#string"/>
  </owl:DatatypeProperty>
  <owl:DatatypeProperty rdf:about="http://example.org/onto/prop/google_compute_router_nat_create">
    <rdfs:label>create</rdfs:label>
    <rdfs:domain rdf:resource="http://example.org/onto/class/google_compute_router_nat"/>
    <rdfs:range rdf:resource="http://www.w3.org/2001/XMLSchema#string"/>
  </owl:DatatypeProperty>
  <owl:DatatypeProperty rdf:about="http://example.org/onto/prop/google_compute_router_nat_delete">
    <rdfs:label>delete</rdfs:label>
    <rdfs:domain rdf:resource="http://example.org/onto/class/google_compute_router_nat"/>
    <rdfs:range rdf:resource="http://www.w3.org/2001/XMLSchema#string"/>
  </owl:DatatypeProperty>
  <owl:DatatypeProperty rdf:about="http://example.org/onto/prop/google_compute_router_nat_update">
    <rdfs:label>update</rdfs:label>
    <rdfs:domain rdf:resource="http://example.org/onto/class/google_compute_router_nat"/>
    <rdfs:range rdf:resource="http://www.w3.org/2001/XMLSchema#string"/>
  </owl:DatatypeProperty>
</rdf:RDF>
