<?xml version="1.0" encoding="UTF-8"?>
<rdf:RDF
  xmlns:rdf="http://www.w3.org/1999/02/22-rdf-syntax-ns#"
  xmlns:rdfs="http://www.w3.org/2000/01/rdf-schema#"
  xmlns:owl="http://www.w3.org/2002/07/owl#"
  xmlns:xsd="http://www.w3.org/2001/XMLSchema#"
  xml:base="http://example.org/onto/">
  <owl:Class rdf:about="http://example.org/onto/class/google_apigee_api_product">
    <rdfs:label>google_apigee_api_product</rdfs:label>
    <rdfs:comment>#
#     ***     AUTO GENERATED CODE    ***    Type: MMv1     ***
#
# ----------------------------------------------------------------------------
#
#     This code is generated by Magic Modules using the following:
#
#     Configuration: https:#github.com/GoogleCloudPlatform/magic-modules/tree/main/mmv1/products/apigee/ApiProduct.yaml
#     Template:      https:#github.com/GoogleCloudPlatform/magic-modules/tree/main/mmv1/templates/terraform/resource.html.markdown.tmpl
#
#     DO NOT EDIT this file directly. Any changes made to this file will be
#     overwritten during the next generation cycle.
#
# ----------------------------------------------------------------------------
subcategory: "Apigee"
description: |-
  An `ApiProduct` in Apigee.
---</rdfs:comment>
  </owl:Class>
  <owl:DatatypeProperty rdf:about="http://example.org/onto/prop/google_apigee_api_product_api_resources">
    <rdfs:label>api_resources</rdfs:label>
    <rdfs:comment>Comma-separated list of API resources to be bundled in the API product. By default, the resource paths are mapped from the proxy.pathsuffix variable.
The proxy path suffix is defined as the URI fragment following the ProxyEndpoint base path. For example, if the apiResources element is defined to be /forecastrss and the base path defined for the API proxy is /weather, then only requests to /weather/forecastrss are permitted by the API product.</rdfs:comment>
    <rdfs:domain rdf:resource="http://example.org/onto/class/google_apigee_api_product"/>
    <rdfs:range rdf:resource="http://www.w3.org/2001/XMLSchema#string"/>
  </owl:DatatypeProperty>
  <owl:DatatypeProperty rdf:about="http://example.org/onto/prop/google_apigee_api_product_approval_type">
    <rdfs:label>approval_type</rdfs:label>
    <rdfs:comment>Flag that specifies how API keys are approved to access the APIs defined by the API product.
Valid values are 'auto' or 'manual'. Possible values: ["auto", "manual"]</rdfs:comment>
    <rdfs:domain rdf:resource="http://example.org/onto/class/google_apigee_api_product"/>
    <rdfs:range rdf:resource="http://www.w3.org/2001/XMLSchema#string"/>
  </owl:DatatypeProperty>
  <owl:DatatypeProperty rdf:about="http://example.org/onto/prop/google_apigee_api_product_created_at">
    <rdfs:label>created_at</rdfs:label>
    <rdfs:comment>Response only. Creation time of this environment as milliseconds since epoch.</rdfs:comment>
    <rdfs:domain rdf:resource="http://example.org/onto/class/google_apigee_api_product"/>
    <rdfs:range rdf:resource="http://www.w3.org/2001/XMLSchema#string"/>
  </owl:DatatypeProperty>
  <owl:DatatypeProperty rdf:about="http://example.org/onto/prop/google_apigee_api_product_description">
    <rdfs:label>description</rdfs:label>
    <rdfs:comment>Description of the API product. Include key information about the API product that is not captured by other fields.</rdfs:comment>
    <rdfs:domain rdf:resource="http://example.org/onto/class/google_apigee_api_product"/>
    <rdfs:range rdf:resource="http://www.w3.org/2001/XMLSchema#string"/>
  </owl:DatatypeProperty>
  <owl:DatatypeProperty rdf:about="http://example.org/onto/prop/google_apigee_api_product_display_name">
    <rdfs:label>display_name</rdfs:label>
    <rdfs:comment>Name displayed in the UI or developer portal to developers registering for API access.</rdfs:comment>
    <rdfs:domain rdf:resource="http://example.org/onto/class/google_apigee_api_product"/>
    <rdfs:range rdf:resource="http://www.w3.org/2001/XMLSchema#string"/>
  </owl:DatatypeProperty>
  <owl:DatatypeProperty rdf:about="http://example.org/onto/prop/google_apigee_api_product_environments">
    <rdfs:label>environments</rdfs:label>
    <rdfs:comment>Comma-separated list of environment names to which the API product is bound. Requests to environments that are not listed are rejected.
By specifying one or more environments, you can bind the resources listed in the API product to a specific environment, preventing developers from accessing those resources through API proxies deployed in another environment.</rdfs:comment>
    <rdfs:domain rdf:resource="http://example.org/onto/class/google_apigee_api_product"/>
    <rdfs:range rdf:resource="http://www.w3.org/2001/XMLSchema#string"/>
  </owl:DatatypeProperty>
  <owl:DatatypeProperty rdf:about="http://example.org/onto/prop/google_apigee_api_product_id">
    <rdfs:label>id</rdfs:label>
    <rdfs:domain rdf:resource="http://example.org/onto/class/google_apigee_api_product"/>
    <rdfs:range rdf:resource="http://www.w3.org/2001/XMLSchema#string"/>
  </owl:DatatypeProperty>
  <owl:DatatypeProperty rdf:about="http://example.org/onto/prop/google_apigee_api_product_last_modified_at">
    <rdfs:label>last_modified_at</rdfs:label>
    <rdfs:comment>Response only. Modified time of this environment as milliseconds since epoch.</rdfs:comment>
    <rdfs:domain rdf:resource="http://example.org/onto/class/google_apigee_api_product"/>
    <rdfs:range rdf:resource="http://www.w3.org/2001/XMLSchema#string"/>
  </owl:DatatypeProperty>
  <owl:DatatypeProperty rdf:about="http://example.org/onto/prop/google_apigee_api_product_name">
    <rdfs:label>name</rdfs:label>
    <rdfs:comment>Internal name of the API product.</rdfs:comment>
    <rdfs:domain rdf:resource="http://example.org/onto/class/google_apigee_api_product"/>
    <rdfs:range rdf:resource="http://www.w3.org/2001/XMLSchema#string"/>
  </owl:DatatypeProperty>
  <owl:DatatypeProperty rdf:about="http://example.org/onto/prop/google_apigee_api_product_org_id">
    <rdfs:label>org_id</rdfs:label>
    <rdfs:comment>The Apigee Organization associated with the Apigee API product,
in the format 'organizations/{{org_name}}'.</rdfs:comment>
    <rdfs:domain rdf:resource="http://example.org/onto/class/google_apigee_api_product"/>
    <rdfs:range rdf:resource="http://www.w3.org/2001/XMLSchema#string"/>
  </owl:DatatypeProperty>
  <owl:DatatypeProperty rdf:about="http://example.org/onto/prop/google_apigee_api_product_proxies">
    <rdfs:label>proxies</rdfs:label>
    <rdfs:comment>Comma-separated list of API proxy names to which this API product is bound. By specifying API proxies, you can associate resources in the API product with specific API proxies, preventing developers from accessing those resources through other API proxies.
Apigee rejects requests to API proxies that are not listed.</rdfs:comment>
    <rdfs:domain rdf:resource="http://example.org/onto/class/google_apigee_api_product"/>
    <rdfs:range rdf:resource="http://www.w3.org/2001/XMLSchema#string"/>
  </owl:DatatypeProperty>
  <owl:DatatypeProperty rdf:about="http://example.org/onto/prop/google_apigee_api_product_quota">
    <rdfs:label>quota</rdfs:label>
    <rdfs:comment>Number of request messages permitted per app by this API product for the specified quotaInterval and quotaTimeUnit.
For example, a quota of 50, for a quotaInterval of 12 and a quotaTimeUnit of hours means 50 requests are allowed every 12 hours.</rdfs:comment>
    <rdfs:domain rdf:resource="http://example.org/onto/class/google_apigee_api_product"/>
    <rdfs:range rdf:resource="http://www.w3.org/2001/XMLSchema#string"/>
  </owl:DatatypeProperty>
  <owl:DatatypeProperty rdf:about="http://example.org/onto/prop/google_apigee_api_product_quota_counter_scope">
    <rdfs:label>quota_counter_scope</rdfs:label>
    <rdfs:comment>Scope of the quota decides how the quota counter gets applied and evaluate for quota violation. If the Scope is set as PROXY, then all the operations defined for the APIproduct that are associated with the same proxy will share the same quota counter set at the APIproduct level, making it a global counter at a proxy level. If the Scope is set as OPERATION, then each operations get the counter set at the API product dedicated, making it a local counter. Note that, the QuotaCounterScope applies only when an operation does not have dedicated quota set for itself. Possible values: ["QUOTA_COUNTER_SCOPE_UNSPECIFIED", "PROXY", "OPERATION"]</rdfs:comment>
    <rdfs:domain rdf:resource="http://example.org/onto/class/google_apigee_api_product"/>
    <rdfs:range rdf:resource="http://www.w3.org/2001/XMLSchema#string"/>
  </owl:DatatypeProperty>
  <owl:DatatypeProperty rdf:about="http://example.org/onto/prop/google_apigee_api_product_quota_interval">
    <rdfs:label>quota_interval</rdfs:label>
    <rdfs:comment>Time interval over which the number of request messages is calculated.</rdfs:comment>
    <rdfs:domain rdf:resource="http://example.org/onto/class/google_apigee_api_product"/>
    <rdfs:range rdf:resource="http://www.w3.org/2001/XMLSchema#string"/>
  </owl:DatatypeProperty>
  <owl:DatatypeProperty rdf:about="http://example.org/onto/prop/google_apigee_api_product_quota_time_unit">
    <rdfs:label>quota_time_unit</rdfs:label>
    <rdfs:comment>Time unit defined for the quotaInterval. Valid values include second, minute, hour, day, month or year.</rdfs:comment>
    <rdfs:domain rdf:resource="http://example.org/onto/class/google_apigee_api_product"/>
    <rdfs:range rdf:resource="http://www.w3.org/2001/XMLSchema#string"/>
  </owl:DatatypeProperty>
  <owl:DatatypeProperty rdf:about="http://example.org/onto/prop/google_apigee_api_product_scopes">
    <rdfs:label>scopes</rdfs:label>
    <rdfs:comment>Comma-separated list of OAuth scopes that are validated at runtime. Apigee validates that the scopes in any access token presented match the scopes defined in the OAuth policy associated with the API product.</rdfs:comment>
    <rdfs:domain rdf:resource="http://example.org/onto/class/google_apigee_api_product"/>
    <rdfs:range rdf:resource="http://www.w3.org/2001/XMLSchema#string"/>
  </owl:DatatypeProperty>
  <owl:DatatypeProperty rdf:about="http://example.org/onto/prop/google_apigee_api_product_space">
    <rdfs:label>space</rdfs:label>
    <rdfs:comment>Optional. The resource ID of the parent Space. If not set, the parent resource will be the Organization.</rdfs:comment>
    <rdfs:domain rdf:resource="http://example.org/onto/class/google_apigee_api_product"/>
    <rdfs:range rdf:resource="http://www.w3.org/2001/XMLSchema#string"/>
  </owl:DatatypeProperty>
  <owl:DatatypeProperty rdf:about="http://example.org/onto/prop/google_apigee_api_product_name">
    <rdfs:label>name</rdfs:label>
    <rdfs:comment>Key of the attribute.</rdfs:comment>
    <rdfs:domain rdf:resource="http://example.org/onto/class/google_apigee_api_product"/>
    <rdfs:range rdf:resource="http://www.w3.org/2001/XMLSchema#string"/>
  </owl:DatatypeProperty>
  <owl:DatatypeProperty rdf:about="http://example.org/onto/prop/google_apigee_api_product_value">
    <rdfs:label>value</rdfs:label>
    <rdfs:comment>Value of the attribute.</rdfs:comment>
    <rdfs:domain rdf:resource="http://example.org/onto/class/google_apigee_api_product"/>
    <rdfs:range rdf:resource="http://www.w3.org/2001/XMLSchema#string"/>
  </owl:DatatypeProperty>
  <owl:DatatypeProperty rdf:about="http://example.org/onto/prop/google_apigee_api_product_operation_config_type">
    <rdfs:label>operation_config_type</rdfs:label>
    <rdfs:comment>Flag that specifes whether the configuration is for Apigee API proxy or a remote service. Valid values include proxy or remoteservice. Defaults to proxy. Set to proxy when Apigee API proxies are associated with the API product. Set to remoteservice when non-Apigee proxies like Istio-Envoy are associated with the API product. Possible values: ["proxy", "remoteservice"]</rdfs:comment>
    <rdfs:domain rdf:resource="http://example.org/onto/class/google_apigee_api_product"/>
    <rdfs:range rdf:resource="http://www.w3.org/2001/XMLSchema#string"/>
  </owl:DatatypeProperty>
  <owl:DatatypeProperty rdf:about="http://example.org/onto/prop/google_apigee_api_product_api_source">
    <rdfs:label>api_source</rdfs:label>
    <rdfs:comment>Required. Name of the API proxy endpoint or remote service with which the GraphQL operation and quota are associated.</rdfs:comment>
    <rdfs:domain rdf:resource="http://example.org/onto/class/google_apigee_api_product"/>
    <rdfs:range rdf:resource="http://www.w3.org/2001/XMLSchema#string"/>
  </owl:DatatypeProperty>
  <owl:DatatypeProperty rdf:about="http://example.org/onto/prop/google_apigee_api_product_name">
    <rdfs:label>name</rdfs:label>
    <rdfs:comment>Key of the attribute.</rdfs:comment>
    <rdfs:domain rdf:resource="http://example.org/onto/class/google_apigee_api_product"/>
    <rdfs:range rdf:resource="http://www.w3.org/2001/XMLSchema#string"/>
  </owl:DatatypeProperty>
  <owl:DatatypeProperty rdf:about="http://example.org/onto/prop/google_apigee_api_product_value">
    <rdfs:label>value</rdfs:label>
    <rdfs:comment>Value of the attribute.</rdfs:comment>
    <rdfs:domain rdf:resource="http://example.org/onto/class/google_apigee_api_product"/>
    <rdfs:range rdf:resource="http://www.w3.org/2001/XMLSchema#string"/>
  </owl:DatatypeProperty>
  <owl:DatatypeProperty rdf:about="http://example.org/onto/prop/google_apigee_api_product_operation">
    <rdfs:label>operation</rdfs:label>
    <rdfs:comment>GraphQL operation name. The name and operation type will be used to apply quotas. If no name is specified, the quota will be applied to all GraphQL operations irrespective of their operation names in the payload.</rdfs:comment>
    <rdfs:domain rdf:resource="http://example.org/onto/class/google_apigee_api_product"/>
    <rdfs:range rdf:resource="http://www.w3.org/2001/XMLSchema#string"/>
  </owl:DatatypeProperty>
  <owl:DatatypeProperty rdf:about="http://example.org/onto/prop/google_apigee_api_product_operation_types">
    <rdfs:label>operation_types</rdfs:label>
    <rdfs:comment>Required. GraphQL operation types. Valid values include query or mutation.
Note: Apigee does not currently support subscription types.</rdfs:comment>
    <rdfs:domain rdf:resource="http://example.org/onto/class/google_apigee_api_product"/>
    <rdfs:range rdf:resource="http://www.w3.org/2001/XMLSchema#string"/>
  </owl:DatatypeProperty>
  <owl:DatatypeProperty rdf:about="http://example.org/onto/prop/google_apigee_api_product_interval">
    <rdfs:label>interval</rdfs:label>
    <rdfs:comment>Required. Time interval over which the number of request messages is calculated.</rdfs:comment>
    <rdfs:domain rdf:resource="http://example.org/onto/class/google_apigee_api_product"/>
    <rdfs:range rdf:resource="http://www.w3.org/2001/XMLSchema#string"/>
  </owl:DatatypeProperty>
  <owl:DatatypeProperty rdf:about="http://example.org/onto/prop/google_apigee_api_product_limit">
    <rdfs:label>limit</rdfs:label>
    <rdfs:comment>Required. Upper limit allowed for the time interval and time unit specified. Requests exceeding this limit will be rejected.</rdfs:comment>
    <rdfs:domain rdf:resource="http://example.org/onto/class/google_apigee_api_product"/>
    <rdfs:range rdf:resource="http://www.w3.org/2001/XMLSchema#string"/>
  </owl:DatatypeProperty>
  <owl:DatatypeProperty rdf:about="http://example.org/onto/prop/google_apigee_api_product_time_unit">
    <rdfs:label>time_unit</rdfs:label>
    <rdfs:comment>Time unit defined for the interval. Valid values include second, minute, hour, day, month or year. If limit and interval are valid, the default value is hour; otherwise, the default is null.</rdfs:comment>
    <rdfs:domain rdf:resource="http://example.org/onto/class/google_apigee_api_product"/>
    <rdfs:range rdf:resource="http://www.w3.org/2001/XMLSchema#string"/>
  </owl:DatatypeProperty>
  <owl:DatatypeProperty rdf:about="http://example.org/onto/prop/google_apigee_api_product_api_source">
    <rdfs:label>api_source</rdfs:label>
    <rdfs:comment>Required. Name of the API proxy with which the gRPC operation and quota are associated.</rdfs:comment>
    <rdfs:domain rdf:resource="http://example.org/onto/class/google_apigee_api_product"/>
    <rdfs:range rdf:resource="http://www.w3.org/2001/XMLSchema#string"/>
  </owl:DatatypeProperty>
  <owl:DatatypeProperty rdf:about="http://example.org/onto/prop/google_apigee_api_product_methods">
    <rdfs:label>methods</rdfs:label>
    <rdfs:comment>List of unqualified gRPC method names for the proxy to which quota will be applied. If this field is empty, the Quota will apply to all operations on the gRPC service defined on the proxy.

Example: Given a proxy that is configured to serve com.petstore.PetService, the methods com.petstore.PetService.ListPets and com.petstore.PetService.GetPet would be specified here as simply ["ListPets", "GetPet"].

Note: Currently, you can specify only a single GraphQLOperation. Specifying more than one will cause the operation to fail.</rdfs:comment>
    <rdfs:domain rdf:resource="http://example.org/onto/class/google_apigee_api_product"/>
    <rdfs:range rdf:resource="http://www.w3.org/2001/XMLSchema#string"/>
  </owl:DatatypeProperty>
  <owl:DatatypeProperty rdf:about="http://example.org/onto/prop/google_apigee_api_product_service">
    <rdfs:label>service</rdfs:label>
    <rdfs:comment>Required. gRPC Service name associated to be associated with the API proxy, on which quota rules can be applied upon.</rdfs:comment>
    <rdfs:domain rdf:resource="http://example.org/onto/class/google_apigee_api_product"/>
    <rdfs:range rdf:resource="http://www.w3.org/2001/XMLSchema#string"/>
  </owl:DatatypeProperty>
  <owl:DatatypeProperty rdf:about="http://example.org/onto/prop/google_apigee_api_product_name">
    <rdfs:label>name</rdfs:label>
    <rdfs:comment>Key of the attribute.</rdfs:comment>
    <rdfs:domain rdf:resource="http://example.org/onto/class/google_apigee_api_product"/>
    <rdfs:range rdf:resource="http://www.w3.org/2001/XMLSchema#string"/>
  </owl:DatatypeProperty>
  <owl:DatatypeProperty rdf:about="http://example.org/onto/prop/google_apigee_api_product_value">
    <rdfs:label>value</rdfs:label>
    <rdfs:comment>Value of the attribute.</rdfs:comment>
    <rdfs:domain rdf:resource="http://example.org/onto/class/google_apigee_api_product"/>
    <rdfs:range rdf:resource="http://www.w3.org/2001/XMLSchema#string"/>
  </owl:DatatypeProperty>
  <owl:DatatypeProperty rdf:about="http://example.org/onto/prop/google_apigee_api_product_interval">
    <rdfs:label>interval</rdfs:label>
    <rdfs:comment>Required. Time interval over which the number of request messages is calculated.</rdfs:comment>
    <rdfs:domain rdf:resource="http://example.org/onto/class/google_apigee_api_product"/>
    <rdfs:range rdf:resource="http://www.w3.org/2001/XMLSchema#string"/>
  </owl:DatatypeProperty>
  <owl:DatatypeProperty rdf:about="http://example.org/onto/prop/google_apigee_api_product_limit">
    <rdfs:label>limit</rdfs:label>
    <rdfs:comment>Required. Upper limit allowed for the time interval and time unit specified. Requests exceeding this limit will be rejected.</rdfs:comment>
    <rdfs:domain rdf:resource="http://example.org/onto/class/google_apigee_api_product"/>
    <rdfs:range rdf:resource="http://www.w3.org/2001/XMLSchema#string"/>
  </owl:DatatypeProperty>
  <owl:DatatypeProperty rdf:about="http://example.org/onto/prop/google_apigee_api_product_time_unit">
    <rdfs:label>time_unit</rdfs:label>
    <rdfs:comment>Time unit defined for the interval. Valid values include second, minute, hour, day, month or year. If limit and interval are valid, the default value is hour; otherwise, the default is null.</rdfs:comment>
    <rdfs:domain rdf:resource="http://example.org/onto/class/google_apigee_api_product"/>
    <rdfs:range rdf:resource="http://www.w3.org/2001/XMLSchema#string"/>
  </owl:DatatypeProperty>
  <owl:DatatypeProperty rdf:about="http://example.org/onto/prop/google_apigee_api_product_operation_config_type">
    <rdfs:label>operation_config_type</rdfs:label>
    <rdfs:comment>Flag that specifes whether the configuration is for Apigee API proxy or a remote service. Valid values include proxy or remoteservice. Defaults to proxy. Set to proxy when Apigee API proxies are associated with the API product. Set to remoteservice when non-Apigee proxies like Istio-Envoy are associated with the API product. Possible values: ["proxy", "remoteservice"]</rdfs:comment>
    <rdfs:domain rdf:resource="http://example.org/onto/class/google_apigee_api_product"/>
    <rdfs:range rdf:resource="http://www.w3.org/2001/XMLSchema#string"/>
  </owl:DatatypeProperty>
  <owl:DatatypeProperty rdf:about="http://example.org/onto/prop/google_apigee_api_product_api_source">
    <rdfs:label>api_source</rdfs:label>
    <rdfs:comment>Required. Name of the API proxy or remote service with which the resources, methods, and quota are associated.</rdfs:comment>
    <rdfs:domain rdf:resource="http://example.org/onto/class/google_apigee_api_product"/>
    <rdfs:range rdf:resource="http://www.w3.org/2001/XMLSchema#string"/>
  </owl:DatatypeProperty>
  <owl:DatatypeProperty rdf:about="http://example.org/onto/prop/google_apigee_api_product_name">
    <rdfs:label>name</rdfs:label>
    <rdfs:comment>Key of the attribute.</rdfs:comment>
    <rdfs:domain rdf:resource="http://example.org/onto/class/google_apigee_api_product"/>
    <rdfs:range rdf:resource="http://www.w3.org/2001/XMLSchema#string"/>
  </owl:DatatypeProperty>
  <owl:DatatypeProperty rdf:about="http://example.org/onto/prop/google_apigee_api_product_value">
    <rdfs:label>value</rdfs:label>
    <rdfs:comment>Value of the attribute.</rdfs:comment>
    <rdfs:domain rdf:resource="http://example.org/onto/class/google_apigee_api_product"/>
    <rdfs:range rdf:resource="http://www.w3.org/2001/XMLSchema#string"/>
  </owl:DatatypeProperty>
  <owl:DatatypeProperty rdf:about="http://example.org/onto/prop/google_apigee_api_product_methods">
    <rdfs:label>methods</rdfs:label>
    <rdfs:comment>Methods refers to the REST verbs, when none specified, all verb types are allowed.</rdfs:comment>
    <rdfs:domain rdf:resource="http://example.org/onto/class/google_apigee_api_product"/>
    <rdfs:range rdf:resource="http://www.w3.org/2001/XMLSchema#string"/>
  </owl:DatatypeProperty>
  <owl:DatatypeProperty rdf:about="http://example.org/onto/prop/google_apigee_api_product_resource">
    <rdfs:label>resource</rdfs:label>
    <rdfs:comment>Required. REST resource path associated with the API proxy or remote service.</rdfs:comment>
    <rdfs:domain rdf:resource="http://example.org/onto/class/google_apigee_api_product"/>
    <rdfs:range rdf:resource="http://www.w3.org/2001/XMLSchema#string"/>
  </owl:DatatypeProperty>
  <owl:DatatypeProperty rdf:about="http://example.org/onto/prop/google_apigee_api_product_interval">
    <rdfs:label>interval</rdfs:label>
    <rdfs:comment>Required. Time interval over which the number of request messages is calculated.</rdfs:comment>
    <rdfs:domain rdf:resource="http://example.org/onto/class/google_apigee_api_product"/>
    <rdfs:range rdf:resource="http://www.w3.org/2001/XMLSchema#string"/>
  </owl:DatatypeProperty>
  <owl:DatatypeProperty rdf:about="http://example.org/onto/prop/google_apigee_api_product_limit">
    <rdfs:label>limit</rdfs:label>
    <rdfs:comment>Required. Upper limit allowed for the time interval and time unit specified. Requests exceeding this limit will be rejected.</rdfs:comment>
    <rdfs:domain rdf:resource="http://example.org/onto/class/google_apigee_api_product"/>
    <rdfs:range rdf:resource="http://www.w3.org/2001/XMLSchema#string"/>
  </owl:DatatypeProperty>
  <owl:DatatypeProperty rdf:about="http://example.org/onto/prop/google_apigee_api_product_time_unit">
    <rdfs:label>time_unit</rdfs:label>
    <rdfs:comment>Time unit defined for the interval. Valid values include second, minute, hour, day, month or year. If limit and interval are valid, the default value is hour; otherwise, the default is null.</rdfs:comment>
    <rdfs:domain rdf:resource="http://example.org/onto/class/google_apigee_api_product"/>
    <rdfs:range rdf:resource="http://www.w3.org/2001/XMLSchema#string"/>
  </owl:DatatypeProperty>
  <owl:DatatypeProperty rdf:about="http://example.org/onto/prop/google_apigee_api_product_create">
    <rdfs:label>create</rdfs:label>
    <rdfs:domain rdf:resource="http://example.org/onto/class/google_apigee_api_product"/>
    <rdfs:range rdf:resource="http://www.w3.org/2001/XMLSchema#string"/>
  </owl:DatatypeProperty>
  <owl:DatatypeProperty rdf:about="http://example.org/onto/prop/google_apigee_api_product_delete">
    <rdfs:label>delete</rdfs:label>
    <rdfs:domain rdf:resource="http://example.org/onto/class/google_apigee_api_product"/>
    <rdfs:range rdf:resource="http://www.w3.org/2001/XMLSchema#string"/>
  </owl:DatatypeProperty>
  <owl:DatatypeProperty rdf:about="http://example.org/onto/prop/google_apigee_api_product_update">
    <rdfs:label>update</rdfs:label>
    <rdfs:domain rdf:resource="http://example.org/onto/class/google_apigee_api_product"/>
    <rdfs:range rdf:resource="http://www.w3.org/2001/XMLSchema#string"/>
  </owl:DatatypeProperty>
</rdf:RDF>
