<?xml version="1.0" encoding="UTF-8"?>
<rdf:RDF
  xmlns:rdf="http://www.w3.org/1999/02/22-rdf-syntax-ns#"
  xmlns:rdfs="http://www.w3.org/2000/01/rdf-schema#"
  xmlns:owl="http://www.w3.org/2002/07/owl#"
  xmlns:xsd="http://www.w3.org/2001/XMLSchema#"
  xml:base="http://example.org/onto/">
  <owl:Class rdf:about="http://example.org/onto/class/google_certificate_manager_certificate">
    <rdfs:label>google_certificate_manager_certificate</rdfs:label>
    <rdfs:comment>#
#     ***     AUTO GENERATED CODE    ***    Type: MMv1     ***
#
# ----------------------------------------------------------------------------
#
#     This code is generated by Magic Modules using the following:
#
#     Configuration: https:#github.com/GoogleCloudPlatform/magic-modules/tree/main/mmv1/products/certificatemanager/Certificate.yaml
#     Template:      https:#github.com/GoogleCloudPlatform/magic-modules/tree/main/mmv1/templates/terraform/resource.html.markdown.tmpl
#
#     DO NOT EDIT this file directly. Any changes made to this file will be
#     overwritten during the next generation cycle.
#
# ----------------------------------------------------------------------------
subcategory: "Certificate Manager"
description: |-
  Certificate represents a HTTP-reachable backend for a Certificate.
---</rdfs:comment>
  </owl:Class>
  <owl:DatatypeProperty rdf:about="http://example.org/onto/prop/google_certificate_manager_certificate_description">
    <rdfs:label>description</rdfs:label>
    <rdfs:comment>A human-readable description of the resource.</rdfs:comment>
    <rdfs:domain rdf:resource="http://example.org/onto/class/google_certificate_manager_certificate"/>
    <rdfs:range rdf:resource="http://www.w3.org/2001/XMLSchema#string"/>
  </owl:DatatypeProperty>
  <owl:DatatypeProperty rdf:about="http://example.org/onto/prop/google_certificate_manager_certificate_effective_labels">
    <rdfs:label>effective_labels</rdfs:label>
    <rdfs:comment>All of labels (key/value pairs) present on the resource in GCP, including the labels configured through Terraform, other clients and services.</rdfs:comment>
    <rdfs:domain rdf:resource="http://example.org/onto/class/google_certificate_manager_certificate"/>
    <rdfs:range rdf:resource="http://www.w3.org/2001/XMLSchema#string"/>
  </owl:DatatypeProperty>
  <owl:DatatypeProperty rdf:about="http://example.org/onto/prop/google_certificate_manager_certificate_id">
    <rdfs:label>id</rdfs:label>
    <rdfs:domain rdf:resource="http://example.org/onto/class/google_certificate_manager_certificate"/>
    <rdfs:range rdf:resource="http://www.w3.org/2001/XMLSchema#string"/>
  </owl:DatatypeProperty>
  <owl:DatatypeProperty rdf:about="http://example.org/onto/prop/google_certificate_manager_certificate_labels">
    <rdfs:label>labels</rdfs:label>
    <rdfs:comment>Set of label tags associated with the Certificate resource.

**Note**: This field is non-authoritative, and will only manage the labels present in your configuration.
Please refer to the field 'effective_labels' for all of the labels present on the resource.</rdfs:comment>
    <rdfs:domain rdf:resource="http://example.org/onto/class/google_certificate_manager_certificate"/>
    <rdfs:range rdf:resource="http://www.w3.org/2001/XMLSchema#string"/>
  </owl:DatatypeProperty>
  <owl:DatatypeProperty rdf:about="http://example.org/onto/prop/google_certificate_manager_certificate_location">
    <rdfs:label>location</rdfs:label>
    <rdfs:comment>The Certificate Manager location. If not specified, "global" is used.</rdfs:comment>
    <rdfs:domain rdf:resource="http://example.org/onto/class/google_certificate_manager_certificate"/>
    <rdfs:range rdf:resource="http://www.w3.org/2001/XMLSchema#string"/>
  </owl:DatatypeProperty>
  <owl:DatatypeProperty rdf:about="http://example.org/onto/prop/google_certificate_manager_certificate_name">
    <rdfs:label>name</rdfs:label>
    <rdfs:comment>A user-defined name of the certificate. Certificate names must be unique
The name must be 1-64 characters long, and match the regular expression [a-zA-Z][a-zA-Z0-9_-]* which means the first character must be a letter,
and all following characters must be a dash, underscore, letter or digit.</rdfs:comment>
    <rdfs:domain rdf:resource="http://example.org/onto/class/google_certificate_manager_certificate"/>
    <rdfs:range rdf:resource="http://www.w3.org/2001/XMLSchema#string"/>
  </owl:DatatypeProperty>
  <owl:DatatypeProperty rdf:about="http://example.org/onto/prop/google_certificate_manager_certificate_project">
    <rdfs:label>project</rdfs:label>
    <rdfs:domain rdf:resource="http://example.org/onto/class/google_certificate_manager_certificate"/>
    <rdfs:range rdf:resource="http://www.w3.org/2001/XMLSchema#string"/>
  </owl:DatatypeProperty>
  <owl:DatatypeProperty rdf:about="http://example.org/onto/prop/google_certificate_manager_certificate_san_dnsnames">
    <rdfs:label>san_dnsnames</rdfs:label>
    <rdfs:comment>The list of Subject Alternative Names of dnsName type defined in the certificate (see RFC 5280 4.2.1.6)</rdfs:comment>
    <rdfs:domain rdf:resource="http://example.org/onto/class/google_certificate_manager_certificate"/>
    <rdfs:range rdf:resource="http://www.w3.org/2001/XMLSchema#string"/>
  </owl:DatatypeProperty>
  <owl:DatatypeProperty rdf:about="http://example.org/onto/prop/google_certificate_manager_certificate_scope">
    <rdfs:label>scope</rdfs:label>
    <rdfs:comment>The scope of the certificate.

DEFAULT: Certificates with default scope are served from core Google data centers.
If unsure, choose this option.

EDGE_CACHE: Certificates with scope EDGE_CACHE are special-purposed certificates, served from Edge Points of Presence.
See https://cloud.google.com/vpc/docs/edge-locations.

ALL_REGIONS: Certificates with ALL_REGIONS scope are served from all GCP regions (You can only use ALL_REGIONS with global certs).
See https://cloud.google.com/compute/docs/regions-zones.

CLIENT_AUTH: Certificates with CLIENT_AUTH scope are used by a load balancer (TLS client) to be presented to the backend (TLS server) when backend mTLS is configured.
See https://cloud.google.com/load-balancing/docs/backend-authenticated-tls-backend-mtls#client-certificate.</rdfs:comment>
    <rdfs:domain rdf:resource="http://example.org/onto/class/google_certificate_manager_certificate"/>
    <rdfs:range rdf:resource="http://www.w3.org/2001/XMLSchema#string"/>
  </owl:DatatypeProperty>
  <owl:DatatypeProperty rdf:about="http://example.org/onto/prop/google_certificate_manager_certificate_terraform_labels">
    <rdfs:label>terraform_labels</rdfs:label>
    <rdfs:comment>The combination of labels configured directly on the resource
 and default labels configured on the provider.</rdfs:comment>
    <rdfs:domain rdf:resource="http://example.org/onto/class/google_certificate_manager_certificate"/>
    <rdfs:range rdf:resource="http://www.w3.org/2001/XMLSchema#string"/>
  </owl:DatatypeProperty>
  <owl:DatatypeProperty rdf:about="http://example.org/onto/prop/google_certificate_manager_certificate_authorization_attempt_info">
    <rdfs:label>authorization_attempt_info</rdfs:label>
    <rdfs:comment>Detailed state of the latest authorization attempt for each domain
specified for this Managed Certificate.</rdfs:comment>
    <rdfs:domain rdf:resource="http://example.org/onto/class/google_certificate_manager_certificate"/>
    <rdfs:range rdf:resource="http://www.w3.org/2001/XMLSchema#string"/>
  </owl:DatatypeProperty>
  <owl:DatatypeProperty rdf:about="http://example.org/onto/prop/google_certificate_manager_certificate_dns_authorizations">
    <rdfs:label>dns_authorizations</rdfs:label>
    <rdfs:comment>Authorizations that will be used for performing domain authorization. Either issuanceConfig or dnsAuthorizations should be specificed, but not both.</rdfs:comment>
    <rdfs:domain rdf:resource="http://example.org/onto/class/google_certificate_manager_certificate"/>
    <rdfs:range rdf:resource="http://www.w3.org/2001/XMLSchema#string"/>
  </owl:DatatypeProperty>
  <owl:DatatypeProperty rdf:about="http://example.org/onto/prop/google_certificate_manager_certificate_domains">
    <rdfs:label>domains</rdfs:label>
    <rdfs:comment>The domains for which a managed SSL certificate will be generated.
Wildcard domains are only supported with DNS challenge resolution</rdfs:comment>
    <rdfs:domain rdf:resource="http://example.org/onto/class/google_certificate_manager_certificate"/>
    <rdfs:range rdf:resource="http://www.w3.org/2001/XMLSchema#string"/>
  </owl:DatatypeProperty>
  <owl:DatatypeProperty rdf:about="http://example.org/onto/prop/google_certificate_manager_certificate_issuance_config">
    <rdfs:label>issuance_config</rdfs:label>
    <rdfs:comment>The resource name for a CertificateIssuanceConfig used to configure private PKI certificates in the format projects/*/locations/*/certificateIssuanceConfigs/*.
If this field is not set, the certificates will instead be publicly signed as documented at https://cloud.google.com/load-balancing/docs/ssl-certificates/google-managed-certs#caa.
Either issuanceConfig or dnsAuthorizations should be specificed, but not both.</rdfs:comment>
    <rdfs:domain rdf:resource="http://example.org/onto/class/google_certificate_manager_certificate"/>
    <rdfs:range rdf:resource="http://www.w3.org/2001/XMLSchema#string"/>
  </owl:DatatypeProperty>
  <owl:DatatypeProperty rdf:about="http://example.org/onto/prop/google_certificate_manager_certificate_provisioning_issue">
    <rdfs:label>provisioning_issue</rdfs:label>
    <rdfs:comment>Information about issues with provisioning this Managed Certificate.</rdfs:comment>
    <rdfs:domain rdf:resource="http://example.org/onto/class/google_certificate_manager_certificate"/>
    <rdfs:range rdf:resource="http://www.w3.org/2001/XMLSchema#string"/>
  </owl:DatatypeProperty>
  <owl:DatatypeProperty rdf:about="http://example.org/onto/prop/google_certificate_manager_certificate_state">
    <rdfs:label>state</rdfs:label>
    <rdfs:comment>A state of this Managed Certificate.</rdfs:comment>
    <rdfs:domain rdf:resource="http://example.org/onto/class/google_certificate_manager_certificate"/>
    <rdfs:range rdf:resource="http://www.w3.org/2001/XMLSchema#string"/>
  </owl:DatatypeProperty>
  <owl:DatatypeProperty rdf:about="http://example.org/onto/prop/google_certificate_manager_certificate_certificate_pem">
    <rdfs:label>certificate_pem</rdfs:label>
    <rdfs:comment>The certificate chain in PEM-encoded form.

Leaf certificate comes first, followed by intermediate ones if any.</rdfs:comment>
    <rdfs:domain rdf:resource="http://example.org/onto/class/google_certificate_manager_certificate"/>
    <rdfs:range rdf:resource="http://www.w3.org/2001/XMLSchema#string"/>
  </owl:DatatypeProperty>
  <owl:DatatypeProperty rdf:about="http://example.org/onto/prop/google_certificate_manager_certificate_pem_certificate">
    <rdfs:label>pem_certificate</rdfs:label>
    <rdfs:comment>The certificate chain in PEM-encoded form.

Leaf certificate comes first, followed by intermediate ones if any.</rdfs:comment>
    <rdfs:domain rdf:resource="http://example.org/onto/class/google_certificate_manager_certificate"/>
    <rdfs:range rdf:resource="http://www.w3.org/2001/XMLSchema#string"/>
  </owl:DatatypeProperty>
  <owl:DatatypeProperty rdf:about="http://example.org/onto/prop/google_certificate_manager_certificate_pem_private_key">
    <rdfs:label>pem_private_key</rdfs:label>
    <rdfs:comment>The private key of the leaf certificate in PEM-encoded form.</rdfs:comment>
    <rdfs:domain rdf:resource="http://example.org/onto/class/google_certificate_manager_certificate"/>
    <rdfs:range rdf:resource="http://www.w3.org/2001/XMLSchema#string"/>
  </owl:DatatypeProperty>
  <owl:DatatypeProperty rdf:about="http://example.org/onto/prop/google_certificate_manager_certificate_private_key_pem">
    <rdfs:label>private_key_pem</rdfs:label>
    <rdfs:comment>The private key of the leaf certificate in PEM-encoded form.</rdfs:comment>
    <rdfs:domain rdf:resource="http://example.org/onto/class/google_certificate_manager_certificate"/>
    <rdfs:range rdf:resource="http://www.w3.org/2001/XMLSchema#string"/>
  </owl:DatatypeProperty>
  <owl:DatatypeProperty rdf:about="http://example.org/onto/prop/google_certificate_manager_certificate_create">
    <rdfs:label>create</rdfs:label>
    <rdfs:domain rdf:resource="http://example.org/onto/class/google_certificate_manager_certificate"/>
    <rdfs:range rdf:resource="http://www.w3.org/2001/XMLSchema#string"/>
  </owl:DatatypeProperty>
  <owl:DatatypeProperty rdf:about="http://example.org/onto/prop/google_certificate_manager_certificate_delete">
    <rdfs:label>delete</rdfs:label>
    <rdfs:domain rdf:resource="http://example.org/onto/class/google_certificate_manager_certificate"/>
    <rdfs:range rdf:resource="http://www.w3.org/2001/XMLSchema#string"/>
  </owl:DatatypeProperty>
  <owl:DatatypeProperty rdf:about="http://example.org/onto/prop/google_certificate_manager_certificate_update">
    <rdfs:label>update</rdfs:label>
    <rdfs:domain rdf:resource="http://example.org/onto/class/google_certificate_manager_certificate"/>
    <rdfs:range rdf:resource="http://www.w3.org/2001/XMLSchema#string"/>
  </owl:DatatypeProperty>
</rdf:RDF>
