<?xml version="1.0" encoding="UTF-8"?>
<rdf:RDF
  xmlns:rdf="http://www.w3.org/1999/02/22-rdf-syntax-ns#"
  xmlns:rdfs="http://www.w3.org/2000/01/rdf-schema#"
  xmlns:owl="http://www.w3.org/2002/07/owl#"
  xmlns:xsd="http://www.w3.org/2001/XMLSchema#"
  xml:base="http://example.org/onto/">
  <owl:Class rdf:about="http://example.org/onto/class/google_essential_contacts_contact">
    <rdfs:label>google_essential_contacts_contact</rdfs:label>
    <rdfs:comment>#
#     ***     AUTO GENERATED CODE    ***    Type: MMv1     ***
#
# ----------------------------------------------------------------------------
#
#     This code is generated by Magic Modules using the following:
#
#     Configuration: https:#github.com/GoogleCloudPlatform/magic-modules/tree/main/mmv1/products/essentialcontacts/Contact.yaml
#     Template:      https:#github.com/GoogleCloudPlatform/magic-modules/tree/main/mmv1/templates/terraform/resource.html.markdown.tmpl
#
#     DO NOT EDIT this file directly. Any changes made to this file will be
#     overwritten during the next generation cycle.
#
# ----------------------------------------------------------------------------
subcategory: "Essential Contacts"
description: |-
  A contact that will receive notifications from Google Cloud.
---</rdfs:comment>
  </owl:Class>
  <owl:DatatypeProperty rdf:about="http://example.org/onto/prop/google_essential_contacts_contact_email">
    <rdfs:label>email</rdfs:label>
    <rdfs:comment>The email address to send notifications to. This does not need to be a Google account.</rdfs:comment>
    <rdfs:domain rdf:resource="http://example.org/onto/class/google_essential_contacts_contact"/>
    <rdfs:range rdf:resource="http://www.w3.org/2001/XMLSchema#string"/>
  </owl:DatatypeProperty>
  <owl:DatatypeProperty rdf:about="http://example.org/onto/prop/google_essential_contacts_contact_id">
    <rdfs:label>id</rdfs:label>
    <rdfs:domain rdf:resource="http://example.org/onto/class/google_essential_contacts_contact"/>
    <rdfs:range rdf:resource="http://www.w3.org/2001/XMLSchema#string"/>
  </owl:DatatypeProperty>
  <owl:DatatypeProperty rdf:about="http://example.org/onto/prop/google_essential_contacts_contact_language_tag">
    <rdfs:label>language_tag</rdfs:label>
    <rdfs:comment>The preferred language for notifications, as a ISO 639-1 language code. See Supported languages for a list of supported languages.</rdfs:comment>
    <rdfs:domain rdf:resource="http://example.org/onto/class/google_essential_contacts_contact"/>
    <rdfs:range rdf:resource="http://www.w3.org/2001/XMLSchema#string"/>
  </owl:DatatypeProperty>
  <owl:DatatypeProperty rdf:about="http://example.org/onto/prop/google_essential_contacts_contact_name">
    <rdfs:label>name</rdfs:label>
    <rdfs:comment>The identifier for the contact. Format: {resourceType}/{resource_id}/contacts/{contact_id}</rdfs:comment>
    <rdfs:domain rdf:resource="http://example.org/onto/class/google_essential_contacts_contact"/>
    <rdfs:range rdf:resource="http://www.w3.org/2001/XMLSchema#string"/>
  </owl:DatatypeProperty>
  <owl:DatatypeProperty rdf:about="http://example.org/onto/prop/google_essential_contacts_contact_notification_category_subscriptions">
    <rdfs:label>notification_category_subscriptions</rdfs:label>
    <rdfs:comment>The categories of notifications that the contact will receive communications for.</rdfs:comment>
    <rdfs:domain rdf:resource="http://example.org/onto/class/google_essential_contacts_contact"/>
    <rdfs:range rdf:resource="http://www.w3.org/2001/XMLSchema#string"/>
  </owl:DatatypeProperty>
  <owl:DatatypeProperty rdf:about="http://example.org/onto/prop/google_essential_contacts_contact_parent">
    <rdfs:label>parent</rdfs:label>
    <rdfs:comment>The resource to save this contact for. Format: organizations/{organization_id}, folders/{folder_id} or projects/{project_id}</rdfs:comment>
    <rdfs:domain rdf:resource="http://example.org/onto/class/google_essential_contacts_contact"/>
    <rdfs:range rdf:resource="http://www.w3.org/2001/XMLSchema#string"/>
  </owl:DatatypeProperty>
  <owl:DatatypeProperty rdf:about="http://example.org/onto/prop/google_essential_contacts_contact_create">
    <rdfs:label>create</rdfs:label>
    <rdfs:domain rdf:resource="http://example.org/onto/class/google_essential_contacts_contact"/>
    <rdfs:range rdf:resource="http://www.w3.org/2001/XMLSchema#string"/>
  </owl:DatatypeProperty>
  <owl:DatatypeProperty rdf:about="http://example.org/onto/prop/google_essential_contacts_contact_delete">
    <rdfs:label>delete</rdfs:label>
    <rdfs:domain rdf:resource="http://example.org/onto/class/google_essential_contacts_contact"/>
    <rdfs:range rdf:resource="http://www.w3.org/2001/XMLSchema#string"/>
  </owl:DatatypeProperty>
  <owl:DatatypeProperty rdf:about="http://example.org/onto/prop/google_essential_contacts_contact_update">
    <rdfs:label>update</rdfs:label>
    <rdfs:domain rdf:resource="http://example.org/onto/class/google_essential_contacts_contact"/>
    <rdfs:range rdf:resource="http://www.w3.org/2001/XMLSchema#string"/>
  </owl:DatatypeProperty>
</rdf:RDF>
