<?xml version="1.0" encoding="UTF-8"?>
<rdf:RDF
  xmlns:rdf="http://www.w3.org/1999/02/22-rdf-syntax-ns#"
  xmlns:rdfs="http://www.w3.org/2000/01/rdf-schema#"
  xmlns:owl="http://www.w3.org/2002/07/owl#"
  xmlns:xsd="http://www.w3.org/2001/XMLSchema#"
  xml:base="http://example.org/onto/">
  <owl:Class rdf:about="http://example.org/onto/class/google_dataproc_gdc_spark_application">
    <rdfs:label>google_dataproc_gdc_spark_application</rdfs:label>
    <rdfs:comment>#
#     ***     AUTO GENERATED CODE    ***    Type: MMv1     ***
#
# ----------------------------------------------------------------------------
#
#     This code is generated by Magic Modules using the following:
#
#     Configuration: https:#github.com/GoogleCloudPlatform/magic-modules/tree/main/mmv1/products/dataprocgdc/SparkApplication.yaml
#     Template:      https:#github.com/GoogleCloudPlatform/magic-modules/tree/main/mmv1/templates/terraform/resource.html.markdown.tmpl
#
#     DO NOT EDIT this file directly. Any changes made to this file will be
#     overwritten during the next generation cycle.
#
# ----------------------------------------------------------------------------
subcategory: "Dataproc on GDC"
description: |-
  A Spark application is a single Spark workload run on a GDC cluster.
---</rdfs:comment>
  </owl:Class>
  <owl:DatatypeProperty rdf:about="http://example.org/onto/prop/google_dataproc_gdc_spark_application_annotations">
    <rdfs:label>annotations</rdfs:label>
    <rdfs:comment>The annotations to associate with this application. Annotations may be used to store client information, but are not used by the server. 

**Note**: This field is non-authoritative, and will only manage the annotations present in your configuration.
Please refer to the field 'effective_annotations' for all of the annotations present on the resource.</rdfs:comment>
    <rdfs:domain rdf:resource="http://example.org/onto/class/google_dataproc_gdc_spark_application"/>
    <rdfs:range rdf:resource="http://www.w3.org/2001/XMLSchema#string"/>
  </owl:DatatypeProperty>
  <owl:DatatypeProperty rdf:about="http://example.org/onto/prop/google_dataproc_gdc_spark_application_application_environment">
    <rdfs:label>application_environment</rdfs:label>
    <rdfs:comment>An ApplicationEnvironment from which to inherit configuration properties.</rdfs:comment>
    <rdfs:domain rdf:resource="http://example.org/onto/class/google_dataproc_gdc_spark_application"/>
    <rdfs:range rdf:resource="http://www.w3.org/2001/XMLSchema#string"/>
  </owl:DatatypeProperty>
  <owl:DatatypeProperty rdf:about="http://example.org/onto/prop/google_dataproc_gdc_spark_application_create_time">
    <rdfs:label>create_time</rdfs:label>
    <rdfs:comment>The timestamp when the resource was created.</rdfs:comment>
    <rdfs:domain rdf:resource="http://example.org/onto/class/google_dataproc_gdc_spark_application"/>
    <rdfs:range rdf:resource="http://www.w3.org/2001/XMLSchema#string"/>
  </owl:DatatypeProperty>
  <owl:DatatypeProperty rdf:about="http://example.org/onto/prop/google_dataproc_gdc_spark_application_dependency_images">
    <rdfs:label>dependency_images</rdfs:label>
    <rdfs:comment>List of container image uris for additional file dependencies. Dependent files are sequentially copied from each image. If a file with the same name exists in 2 images then the file from later image is used.</rdfs:comment>
    <rdfs:domain rdf:resource="http://example.org/onto/class/google_dataproc_gdc_spark_application"/>
    <rdfs:range rdf:resource="http://www.w3.org/2001/XMLSchema#string"/>
  </owl:DatatypeProperty>
  <owl:DatatypeProperty rdf:about="http://example.org/onto/prop/google_dataproc_gdc_spark_application_display_name">
    <rdfs:label>display_name</rdfs:label>
    <rdfs:comment>User-provided human-readable name to be used in user interfaces.</rdfs:comment>
    <rdfs:domain rdf:resource="http://example.org/onto/class/google_dataproc_gdc_spark_application"/>
    <rdfs:range rdf:resource="http://www.w3.org/2001/XMLSchema#string"/>
  </owl:DatatypeProperty>
  <owl:DatatypeProperty rdf:about="http://example.org/onto/prop/google_dataproc_gdc_spark_application_effective_annotations">
    <rdfs:label>effective_annotations</rdfs:label>
    <rdfs:comment>All of annotations (key/value pairs) present on the resource in GCP, including the annotations configured through Terraform, other clients and services.</rdfs:comment>
    <rdfs:domain rdf:resource="http://example.org/onto/class/google_dataproc_gdc_spark_application"/>
    <rdfs:range rdf:resource="http://www.w3.org/2001/XMLSchema#string"/>
  </owl:DatatypeProperty>
  <owl:DatatypeProperty rdf:about="http://example.org/onto/prop/google_dataproc_gdc_spark_application_effective_labels">
    <rdfs:label>effective_labels</rdfs:label>
    <rdfs:comment>All of labels (key/value pairs) present on the resource in GCP, including the labels configured through Terraform, other clients and services.</rdfs:comment>
    <rdfs:domain rdf:resource="http://example.org/onto/class/google_dataproc_gdc_spark_application"/>
    <rdfs:range rdf:resource="http://www.w3.org/2001/XMLSchema#string"/>
  </owl:DatatypeProperty>
  <owl:DatatypeProperty rdf:about="http://example.org/onto/prop/google_dataproc_gdc_spark_application_id">
    <rdfs:label>id</rdfs:label>
    <rdfs:domain rdf:resource="http://example.org/onto/class/google_dataproc_gdc_spark_application"/>
    <rdfs:range rdf:resource="http://www.w3.org/2001/XMLSchema#string"/>
  </owl:DatatypeProperty>
  <owl:DatatypeProperty rdf:about="http://example.org/onto/prop/google_dataproc_gdc_spark_application_labels">
    <rdfs:label>labels</rdfs:label>
    <rdfs:comment>The labels to associate with this application. Labels may be used for filtering and billing tracking. 

**Note**: This field is non-authoritative, and will only manage the labels present in your configuration.
Please refer to the field 'effective_labels' for all of the labels present on the resource.</rdfs:comment>
    <rdfs:domain rdf:resource="http://example.org/onto/class/google_dataproc_gdc_spark_application"/>
    <rdfs:range rdf:resource="http://www.w3.org/2001/XMLSchema#string"/>
  </owl:DatatypeProperty>
  <owl:DatatypeProperty rdf:about="http://example.org/onto/prop/google_dataproc_gdc_spark_application_location">
    <rdfs:label>location</rdfs:label>
    <rdfs:comment>The location of the spark application.</rdfs:comment>
    <rdfs:domain rdf:resource="http://example.org/onto/class/google_dataproc_gdc_spark_application"/>
    <rdfs:range rdf:resource="http://www.w3.org/2001/XMLSchema#string"/>
  </owl:DatatypeProperty>
  <owl:DatatypeProperty rdf:about="http://example.org/onto/prop/google_dataproc_gdc_spark_application_monitoring_endpoint">
    <rdfs:label>monitoring_endpoint</rdfs:label>
    <rdfs:comment>URL for a monitoring UI for this application (for eventual Spark PHS/UI support) Out of scope for private GA</rdfs:comment>
    <rdfs:domain rdf:resource="http://example.org/onto/class/google_dataproc_gdc_spark_application"/>
    <rdfs:range rdf:resource="http://www.w3.org/2001/XMLSchema#string"/>
  </owl:DatatypeProperty>
  <owl:DatatypeProperty rdf:about="http://example.org/onto/prop/google_dataproc_gdc_spark_application_name">
    <rdfs:label>name</rdfs:label>
    <rdfs:comment>Identifier. The name of the application. Format: projects/{project}/locations/{location}/serviceInstances/{service_instance}/sparkApplications/{application}</rdfs:comment>
    <rdfs:domain rdf:resource="http://example.org/onto/class/google_dataproc_gdc_spark_application"/>
    <rdfs:range rdf:resource="http://www.w3.org/2001/XMLSchema#string"/>
  </owl:DatatypeProperty>
  <owl:DatatypeProperty rdf:about="http://example.org/onto/prop/google_dataproc_gdc_spark_application_namespace">
    <rdfs:label>namespace</rdfs:label>
    <rdfs:comment>The Kubernetes namespace in which to create the application. This namespace must already exist on the cluster.</rdfs:comment>
    <rdfs:domain rdf:resource="http://example.org/onto/class/google_dataproc_gdc_spark_application"/>
    <rdfs:range rdf:resource="http://www.w3.org/2001/XMLSchema#string"/>
  </owl:DatatypeProperty>
  <owl:DatatypeProperty rdf:about="http://example.org/onto/prop/google_dataproc_gdc_spark_application_output_uri">
    <rdfs:label>output_uri</rdfs:label>
    <rdfs:comment>An HCFS URI pointing to the location of stdout and stdout of the application Mainly useful for Pantheon and gcloud Not in scope for private GA</rdfs:comment>
    <rdfs:domain rdf:resource="http://example.org/onto/class/google_dataproc_gdc_spark_application"/>
    <rdfs:range rdf:resource="http://www.w3.org/2001/XMLSchema#string"/>
  </owl:DatatypeProperty>
  <owl:DatatypeProperty rdf:about="http://example.org/onto/prop/google_dataproc_gdc_spark_application_project">
    <rdfs:label>project</rdfs:label>
    <rdfs:domain rdf:resource="http://example.org/onto/class/google_dataproc_gdc_spark_application"/>
    <rdfs:range rdf:resource="http://www.w3.org/2001/XMLSchema#string"/>
  </owl:DatatypeProperty>
  <owl:DatatypeProperty rdf:about="http://example.org/onto/prop/google_dataproc_gdc_spark_application_properties">
    <rdfs:label>properties</rdfs:label>
    <rdfs:comment>application-specific properties.</rdfs:comment>
    <rdfs:domain rdf:resource="http://example.org/onto/class/google_dataproc_gdc_spark_application"/>
    <rdfs:range rdf:resource="http://www.w3.org/2001/XMLSchema#string"/>
  </owl:DatatypeProperty>
  <owl:DatatypeProperty rdf:about="http://example.org/onto/prop/google_dataproc_gdc_spark_application_reconciling">
    <rdfs:label>reconciling</rdfs:label>
    <rdfs:comment>Whether the application is currently reconciling. True if the current state of the resource does not match the intended state, and the system is working to reconcile them, whether or not the change was user initiated.</rdfs:comment>
    <rdfs:domain rdf:resource="http://example.org/onto/class/google_dataproc_gdc_spark_application"/>
    <rdfs:range rdf:resource="http://www.w3.org/2001/XMLSchema#string"/>
  </owl:DatatypeProperty>
  <owl:DatatypeProperty rdf:about="http://example.org/onto/prop/google_dataproc_gdc_spark_application_serviceinstance">
    <rdfs:label>serviceinstance</rdfs:label>
    <rdfs:comment>The id of the service instance to which this spark application belongs.</rdfs:comment>
    <rdfs:domain rdf:resource="http://example.org/onto/class/google_dataproc_gdc_spark_application"/>
    <rdfs:range rdf:resource="http://www.w3.org/2001/XMLSchema#string"/>
  </owl:DatatypeProperty>
  <owl:DatatypeProperty rdf:about="http://example.org/onto/prop/google_dataproc_gdc_spark_application_spark_application_id">
    <rdfs:label>spark_application_id</rdfs:label>
    <rdfs:comment>The id of the application</rdfs:comment>
    <rdfs:domain rdf:resource="http://example.org/onto/class/google_dataproc_gdc_spark_application"/>
    <rdfs:range rdf:resource="http://www.w3.org/2001/XMLSchema#string"/>
  </owl:DatatypeProperty>
  <owl:DatatypeProperty rdf:about="http://example.org/onto/prop/google_dataproc_gdc_spark_application_state">
    <rdfs:label>state</rdfs:label>
    <rdfs:comment>The current state.
Possible values:
* 'STATE_UNSPECIFIED'
* 'PENDING'
* 'RUNNING'
* 'CANCELLING'
* 'CANCELLED'
* 'SUCCEEDED'
* 'FAILED'</rdfs:comment>
    <rdfs:domain rdf:resource="http://example.org/onto/class/google_dataproc_gdc_spark_application"/>
    <rdfs:range rdf:resource="http://www.w3.org/2001/XMLSchema#string"/>
  </owl:DatatypeProperty>
  <owl:DatatypeProperty rdf:about="http://example.org/onto/prop/google_dataproc_gdc_spark_application_state_message">
    <rdfs:label>state_message</rdfs:label>
    <rdfs:comment>A message explaining the current state.</rdfs:comment>
    <rdfs:domain rdf:resource="http://example.org/onto/class/google_dataproc_gdc_spark_application"/>
    <rdfs:range rdf:resource="http://www.w3.org/2001/XMLSchema#string"/>
  </owl:DatatypeProperty>
  <owl:DatatypeProperty rdf:about="http://example.org/onto/prop/google_dataproc_gdc_spark_application_terraform_labels">
    <rdfs:label>terraform_labels</rdfs:label>
    <rdfs:comment>The combination of labels configured directly on the resource
 and default labels configured on the provider.</rdfs:comment>
    <rdfs:domain rdf:resource="http://example.org/onto/class/google_dataproc_gdc_spark_application"/>
    <rdfs:range rdf:resource="http://www.w3.org/2001/XMLSchema#string"/>
  </owl:DatatypeProperty>
  <owl:DatatypeProperty rdf:about="http://example.org/onto/prop/google_dataproc_gdc_spark_application_uid">
    <rdfs:label>uid</rdfs:label>
    <rdfs:comment>System generated unique identifier for this application, formatted as UUID4.</rdfs:comment>
    <rdfs:domain rdf:resource="http://example.org/onto/class/google_dataproc_gdc_spark_application"/>
    <rdfs:range rdf:resource="http://www.w3.org/2001/XMLSchema#string"/>
  </owl:DatatypeProperty>
  <owl:DatatypeProperty rdf:about="http://example.org/onto/prop/google_dataproc_gdc_spark_application_update_time">
    <rdfs:label>update_time</rdfs:label>
    <rdfs:comment>The timestamp when the resource was most recently updated.</rdfs:comment>
    <rdfs:domain rdf:resource="http://example.org/onto/class/google_dataproc_gdc_spark_application"/>
    <rdfs:range rdf:resource="http://www.w3.org/2001/XMLSchema#string"/>
  </owl:DatatypeProperty>
  <owl:DatatypeProperty rdf:about="http://example.org/onto/prop/google_dataproc_gdc_spark_application_version">
    <rdfs:label>version</rdfs:label>
    <rdfs:comment>The Dataproc version of this application.</rdfs:comment>
    <rdfs:domain rdf:resource="http://example.org/onto/class/google_dataproc_gdc_spark_application"/>
    <rdfs:range rdf:resource="http://www.w3.org/2001/XMLSchema#string"/>
  </owl:DatatypeProperty>
  <owl:DatatypeProperty rdf:about="http://example.org/onto/prop/google_dataproc_gdc_spark_application_archive_uris">
    <rdfs:label>archive_uris</rdfs:label>
    <rdfs:comment>HCFS URIs of archives to be extracted into the working directory of each executor. Supported file types: .jar, .tar, .tar.gz, .tgz, and .zip.</rdfs:comment>
    <rdfs:domain rdf:resource="http://example.org/onto/class/google_dataproc_gdc_spark_application"/>
    <rdfs:range rdf:resource="http://www.w3.org/2001/XMLSchema#string"/>
  </owl:DatatypeProperty>
  <owl:DatatypeProperty rdf:about="http://example.org/onto/prop/google_dataproc_gdc_spark_application_args">
    <rdfs:label>args</rdfs:label>
    <rdfs:comment>The arguments to pass to the driver.  Do not include arguments, such as '--conf', that can be set as job properties, since a collision may occur that causes an incorrect job submission.</rdfs:comment>
    <rdfs:domain rdf:resource="http://example.org/onto/class/google_dataproc_gdc_spark_application"/>
    <rdfs:range rdf:resource="http://www.w3.org/2001/XMLSchema#string"/>
  </owl:DatatypeProperty>
  <owl:DatatypeProperty rdf:about="http://example.org/onto/prop/google_dataproc_gdc_spark_application_file_uris">
    <rdfs:label>file_uris</rdfs:label>
    <rdfs:comment>HCFS URIs of files to be placed in the working directory of each executor. Useful for naively parallel tasks.</rdfs:comment>
    <rdfs:domain rdf:resource="http://example.org/onto/class/google_dataproc_gdc_spark_application"/>
    <rdfs:range rdf:resource="http://www.w3.org/2001/XMLSchema#string"/>
  </owl:DatatypeProperty>
  <owl:DatatypeProperty rdf:about="http://example.org/onto/prop/google_dataproc_gdc_spark_application_jar_file_uris">
    <rdfs:label>jar_file_uris</rdfs:label>
    <rdfs:comment>HCFS URIs of jar files to add to the CLASSPATHs of the Python driver and tasks.</rdfs:comment>
    <rdfs:domain rdf:resource="http://example.org/onto/class/google_dataproc_gdc_spark_application"/>
    <rdfs:range rdf:resource="http://www.w3.org/2001/XMLSchema#string"/>
  </owl:DatatypeProperty>
  <owl:DatatypeProperty rdf:about="http://example.org/onto/prop/google_dataproc_gdc_spark_application_main_python_file_uri">
    <rdfs:label>main_python_file_uri</rdfs:label>
    <rdfs:comment>The HCFS URI of the main Python file to use as the driver. Must be a .py file.</rdfs:comment>
    <rdfs:domain rdf:resource="http://example.org/onto/class/google_dataproc_gdc_spark_application"/>
    <rdfs:range rdf:resource="http://www.w3.org/2001/XMLSchema#string"/>
  </owl:DatatypeProperty>
  <owl:DatatypeProperty rdf:about="http://example.org/onto/prop/google_dataproc_gdc_spark_application_python_file_uris">
    <rdfs:label>python_file_uris</rdfs:label>
    <rdfs:comment>HCFS file URIs of Python files to pass to the PySpark framework. Supported file types: .py, .egg, and .zip.</rdfs:comment>
    <rdfs:domain rdf:resource="http://example.org/onto/class/google_dataproc_gdc_spark_application"/>
    <rdfs:range rdf:resource="http://www.w3.org/2001/XMLSchema#string"/>
  </owl:DatatypeProperty>
  <owl:DatatypeProperty rdf:about="http://example.org/onto/prop/google_dataproc_gdc_spark_application_archive_uris">
    <rdfs:label>archive_uris</rdfs:label>
    <rdfs:comment>HCFS URIs of archives to be extracted into the working directory of each executor. Supported file types: '.jar', '.tar', '.tar.gz', '.tgz', and '.zip'.</rdfs:comment>
    <rdfs:domain rdf:resource="http://example.org/onto/class/google_dataproc_gdc_spark_application"/>
    <rdfs:range rdf:resource="http://www.w3.org/2001/XMLSchema#string"/>
  </owl:DatatypeProperty>
  <owl:DatatypeProperty rdf:about="http://example.org/onto/prop/google_dataproc_gdc_spark_application_args">
    <rdfs:label>args</rdfs:label>
    <rdfs:comment>The arguments to pass to the driver. Do not include arguments that can be set as application properties, such as '--conf', since a collision can occur that causes an incorrect application submission.</rdfs:comment>
    <rdfs:domain rdf:resource="http://example.org/onto/class/google_dataproc_gdc_spark_application"/>
    <rdfs:range rdf:resource="http://www.w3.org/2001/XMLSchema#string"/>
  </owl:DatatypeProperty>
  <owl:DatatypeProperty rdf:about="http://example.org/onto/prop/google_dataproc_gdc_spark_application_file_uris">
    <rdfs:label>file_uris</rdfs:label>
    <rdfs:comment>HCFS URIs of files to be placed in the working directory of each executor.</rdfs:comment>
    <rdfs:domain rdf:resource="http://example.org/onto/class/google_dataproc_gdc_spark_application"/>
    <rdfs:range rdf:resource="http://www.w3.org/2001/XMLSchema#string"/>
  </owl:DatatypeProperty>
  <owl:DatatypeProperty rdf:about="http://example.org/onto/prop/google_dataproc_gdc_spark_application_jar_file_uris">
    <rdfs:label>jar_file_uris</rdfs:label>
    <rdfs:comment>HCFS URIs of jar files to add to the classpath of the Spark driver and tasks.</rdfs:comment>
    <rdfs:domain rdf:resource="http://example.org/onto/class/google_dataproc_gdc_spark_application"/>
    <rdfs:range rdf:resource="http://www.w3.org/2001/XMLSchema#string"/>
  </owl:DatatypeProperty>
  <owl:DatatypeProperty rdf:about="http://example.org/onto/prop/google_dataproc_gdc_spark_application_main_class">
    <rdfs:label>main_class</rdfs:label>
    <rdfs:comment>The name of the driver main class. The jar file that contains the class must be in the classpath or specified in 'jar_file_uris'.</rdfs:comment>
    <rdfs:domain rdf:resource="http://example.org/onto/class/google_dataproc_gdc_spark_application"/>
    <rdfs:range rdf:resource="http://www.w3.org/2001/XMLSchema#string"/>
  </owl:DatatypeProperty>
  <owl:DatatypeProperty rdf:about="http://example.org/onto/prop/google_dataproc_gdc_spark_application_main_jar_file_uri">
    <rdfs:label>main_jar_file_uri</rdfs:label>
    <rdfs:comment>The HCFS URI of the jar file that contains the main class.</rdfs:comment>
    <rdfs:domain rdf:resource="http://example.org/onto/class/google_dataproc_gdc_spark_application"/>
    <rdfs:range rdf:resource="http://www.w3.org/2001/XMLSchema#string"/>
  </owl:DatatypeProperty>
  <owl:DatatypeProperty rdf:about="http://example.org/onto/prop/google_dataproc_gdc_spark_application_archive_uris">
    <rdfs:label>archive_uris</rdfs:label>
    <rdfs:comment>HCFS URIs of archives to be extracted into the working directory of each executor. Supported file types: .jar, .tar, .tar.gz, .tgz, and .zip.</rdfs:comment>
    <rdfs:domain rdf:resource="http://example.org/onto/class/google_dataproc_gdc_spark_application"/>
    <rdfs:range rdf:resource="http://www.w3.org/2001/XMLSchema#string"/>
  </owl:DatatypeProperty>
  <owl:DatatypeProperty rdf:about="http://example.org/onto/prop/google_dataproc_gdc_spark_application_args">
    <rdfs:label>args</rdfs:label>
    <rdfs:comment>The arguments to pass to the driver.  Do not include arguments, such as '--conf', that can be set as job properties, since a collision may occur that causes an incorrect job submission.</rdfs:comment>
    <rdfs:domain rdf:resource="http://example.org/onto/class/google_dataproc_gdc_spark_application"/>
    <rdfs:range rdf:resource="http://www.w3.org/2001/XMLSchema#string"/>
  </owl:DatatypeProperty>
  <owl:DatatypeProperty rdf:about="http://example.org/onto/prop/google_dataproc_gdc_spark_application_file_uris">
    <rdfs:label>file_uris</rdfs:label>
    <rdfs:comment>HCFS URIs of files to be placed in the working directory of each executor. Useful for naively parallel tasks.</rdfs:comment>
    <rdfs:domain rdf:resource="http://example.org/onto/class/google_dataproc_gdc_spark_application"/>
    <rdfs:range rdf:resource="http://www.w3.org/2001/XMLSchema#string"/>
  </owl:DatatypeProperty>
  <owl:DatatypeProperty rdf:about="http://example.org/onto/prop/google_dataproc_gdc_spark_application_main_r_file_uri">
    <rdfs:label>main_r_file_uri</rdfs:label>
    <rdfs:comment>The HCFS URI of the main R file to use as the driver. Must be a .R file.</rdfs:comment>
    <rdfs:domain rdf:resource="http://example.org/onto/class/google_dataproc_gdc_spark_application"/>
    <rdfs:range rdf:resource="http://www.w3.org/2001/XMLSchema#string"/>
  </owl:DatatypeProperty>
  <owl:DatatypeProperty rdf:about="http://example.org/onto/prop/google_dataproc_gdc_spark_application_jar_file_uris">
    <rdfs:label>jar_file_uris</rdfs:label>
    <rdfs:comment>HCFS URIs of jar files to be added to the Spark CLASSPATH.</rdfs:comment>
    <rdfs:domain rdf:resource="http://example.org/onto/class/google_dataproc_gdc_spark_application"/>
    <rdfs:range rdf:resource="http://www.w3.org/2001/XMLSchema#string"/>
  </owl:DatatypeProperty>
  <owl:DatatypeProperty rdf:about="http://example.org/onto/prop/google_dataproc_gdc_spark_application_query_file_uri">
    <rdfs:label>query_file_uri</rdfs:label>
    <rdfs:comment>The HCFS URI of the script that contains SQL queries.</rdfs:comment>
    <rdfs:domain rdf:resource="http://example.org/onto/class/google_dataproc_gdc_spark_application"/>
    <rdfs:range rdf:resource="http://www.w3.org/2001/XMLSchema#string"/>
  </owl:DatatypeProperty>
  <owl:DatatypeProperty rdf:about="http://example.org/onto/prop/google_dataproc_gdc_spark_application_script_variables">
    <rdfs:label>script_variables</rdfs:label>
    <rdfs:comment>Mapping of query variable names to values (equivalent to the Spark SQL command: SET 'name="value";').</rdfs:comment>
    <rdfs:domain rdf:resource="http://example.org/onto/class/google_dataproc_gdc_spark_application"/>
    <rdfs:range rdf:resource="http://www.w3.org/2001/XMLSchema#string"/>
  </owl:DatatypeProperty>
  <owl:DatatypeProperty rdf:about="http://example.org/onto/prop/google_dataproc_gdc_spark_application_queries">
    <rdfs:label>queries</rdfs:label>
    <rdfs:comment>The queries to run.</rdfs:comment>
    <rdfs:domain rdf:resource="http://example.org/onto/class/google_dataproc_gdc_spark_application"/>
    <rdfs:range rdf:resource="http://www.w3.org/2001/XMLSchema#string"/>
  </owl:DatatypeProperty>
  <owl:DatatypeProperty rdf:about="http://example.org/onto/prop/google_dataproc_gdc_spark_application_create">
    <rdfs:label>create</rdfs:label>
    <rdfs:domain rdf:resource="http://example.org/onto/class/google_dataproc_gdc_spark_application"/>
    <rdfs:range rdf:resource="http://www.w3.org/2001/XMLSchema#string"/>
  </owl:DatatypeProperty>
  <owl:DatatypeProperty rdf:about="http://example.org/onto/prop/google_dataproc_gdc_spark_application_delete">
    <rdfs:label>delete</rdfs:label>
    <rdfs:domain rdf:resource="http://example.org/onto/class/google_dataproc_gdc_spark_application"/>
    <rdfs:range rdf:resource="http://www.w3.org/2001/XMLSchema#string"/>
  </owl:DatatypeProperty>
  <owl:DatatypeProperty rdf:about="http://example.org/onto/prop/google_dataproc_gdc_spark_application_update">
    <rdfs:label>update</rdfs:label>
    <rdfs:domain rdf:resource="http://example.org/onto/class/google_dataproc_gdc_spark_application"/>
    <rdfs:range rdf:resource="http://www.w3.org/2001/XMLSchema#string"/>
  </owl:DatatypeProperty>
</rdf:RDF>
