<?xml version="1.0" encoding="UTF-8"?>
<rdf:RDF
  xmlns:rdf="http://www.w3.org/1999/02/22-rdf-syntax-ns#"
  xmlns:rdfs="http://www.w3.org/2000/01/rdf-schema#"
  xmlns:owl="http://www.w3.org/2002/07/owl#"
  xmlns:xsd="http://www.w3.org/2001/XMLSchema#"
  xml:base="http://example.org/onto/">
  <owl:Class rdf:about="http://example.org/onto/class/google_beyondcorp_security_gateway">
    <rdfs:label>google_beyondcorp_security_gateway</rdfs:label>
    <rdfs:comment>#
#     ***     AUTO GENERATED CODE    ***    Type: MMv1     ***
#
# ----------------------------------------------------------------------------
#
#     This code is generated by Magic Modules using the following:
#
#     Configuration: https:#github.com/GoogleCloudPlatform/magic-modules/tree/main/mmv1/products/beyondcorp/SecurityGateway.yaml
#     Template:      https:#github.com/GoogleCloudPlatform/magic-modules/tree/main/mmv1/templates/terraform/resource.html.markdown.tmpl
#
#     DO NOT EDIT this file directly. Any changes made to this file will be
#     overwritten during the next generation cycle.
#
# ----------------------------------------------------------------------------
subcategory: "BeyondCorp"
description: |-
  Deployment of Security Gateway.
---</rdfs:comment>
  </owl:Class>
  <owl:DatatypeProperty rdf:about="http://example.org/onto/prop/google_beyondcorp_security_gateway_create_time">
    <rdfs:label>create_time</rdfs:label>
    <rdfs:comment>Output only. Timestamp when the resource was created.</rdfs:comment>
    <rdfs:domain rdf:resource="http://example.org/onto/class/google_beyondcorp_security_gateway"/>
    <rdfs:range rdf:resource="http://www.w3.org/2001/XMLSchema#string"/>
  </owl:DatatypeProperty>
  <owl:DatatypeProperty rdf:about="http://example.org/onto/prop/google_beyondcorp_security_gateway_delegating_service_account">
    <rdfs:label>delegating_service_account</rdfs:label>
    <rdfs:comment>Service account used for operations that involve resources in consumer projects.</rdfs:comment>
    <rdfs:domain rdf:resource="http://example.org/onto/class/google_beyondcorp_security_gateway"/>
    <rdfs:range rdf:resource="http://www.w3.org/2001/XMLSchema#string"/>
  </owl:DatatypeProperty>
  <owl:DatatypeProperty rdf:about="http://example.org/onto/prop/google_beyondcorp_security_gateway_display_name">
    <rdfs:label>display_name</rdfs:label>
    <rdfs:comment>Optional. An arbitrary user-provided name for the SecurityGateway.
Cannot exceed 64 characters.</rdfs:comment>
    <rdfs:domain rdf:resource="http://example.org/onto/class/google_beyondcorp_security_gateway"/>
    <rdfs:range rdf:resource="http://www.w3.org/2001/XMLSchema#string"/>
  </owl:DatatypeProperty>
  <owl:DatatypeProperty rdf:about="http://example.org/onto/prop/google_beyondcorp_security_gateway_external_ips">
    <rdfs:label>external_ips</rdfs:label>
    <rdfs:comment>Output only. IP addresses that will be used for establishing
connection to the endpoints.</rdfs:comment>
    <rdfs:domain rdf:resource="http://example.org/onto/class/google_beyondcorp_security_gateway"/>
    <rdfs:range rdf:resource="http://www.w3.org/2001/XMLSchema#string"/>
  </owl:DatatypeProperty>
  <owl:DatatypeProperty rdf:about="http://example.org/onto/prop/google_beyondcorp_security_gateway_id">
    <rdfs:label>id</rdfs:label>
    <rdfs:domain rdf:resource="http://example.org/onto/class/google_beyondcorp_security_gateway"/>
    <rdfs:range rdf:resource="http://www.w3.org/2001/XMLSchema#string"/>
  </owl:DatatypeProperty>
  <owl:DatatypeProperty rdf:about="http://example.org/onto/prop/google_beyondcorp_security_gateway_location">
    <rdfs:label>location</rdfs:label>
    <rdfs:comment>Resource ID segment making up resource 'name'. It identifies the resource within its parent collection as described in https://google.aip.dev/122. Must be omitted or set to 'global'.</rdfs:comment>
    <rdfs:domain rdf:resource="http://example.org/onto/class/google_beyondcorp_security_gateway"/>
    <rdfs:range rdf:resource="http://www.w3.org/2001/XMLSchema#string"/>
  </owl:DatatypeProperty>
  <owl:DatatypeProperty rdf:about="http://example.org/onto/prop/google_beyondcorp_security_gateway_name">
    <rdfs:label>name</rdfs:label>
    <rdfs:comment>Identifier. Name of the resource.</rdfs:comment>
    <rdfs:domain rdf:resource="http://example.org/onto/class/google_beyondcorp_security_gateway"/>
    <rdfs:range rdf:resource="http://www.w3.org/2001/XMLSchema#string"/>
  </owl:DatatypeProperty>
  <owl:DatatypeProperty rdf:about="http://example.org/onto/prop/google_beyondcorp_security_gateway_project">
    <rdfs:label>project</rdfs:label>
    <rdfs:domain rdf:resource="http://example.org/onto/class/google_beyondcorp_security_gateway"/>
    <rdfs:range rdf:resource="http://www.w3.org/2001/XMLSchema#string"/>
  </owl:DatatypeProperty>
  <owl:DatatypeProperty rdf:about="http://example.org/onto/prop/google_beyondcorp_security_gateway_security_gateway_id">
    <rdfs:label>security_gateway_id</rdfs:label>
    <rdfs:comment>Optional. User-settable SecurityGateway resource ID.
* Must start with a letter.
* Must contain between 4-63 characters from '/a-z-/'.
* Must end with a number or letter.</rdfs:comment>
    <rdfs:domain rdf:resource="http://example.org/onto/class/google_beyondcorp_security_gateway"/>
    <rdfs:range rdf:resource="http://www.w3.org/2001/XMLSchema#string"/>
  </owl:DatatypeProperty>
  <owl:DatatypeProperty rdf:about="http://example.org/onto/prop/google_beyondcorp_security_gateway_state">
    <rdfs:label>state</rdfs:label>
    <rdfs:comment>Output only. The operational state of the SecurityGateway.
Possible values:
STATE_UNSPECIFIED
CREATING
UPDATING
DELETING
RUNNING
DOWN
ERROR</rdfs:comment>
    <rdfs:domain rdf:resource="http://example.org/onto/class/google_beyondcorp_security_gateway"/>
    <rdfs:range rdf:resource="http://www.w3.org/2001/XMLSchema#string"/>
  </owl:DatatypeProperty>
  <owl:DatatypeProperty rdf:about="http://example.org/onto/prop/google_beyondcorp_security_gateway_update_time">
    <rdfs:label>update_time</rdfs:label>
    <rdfs:comment>Output only. Timestamp when the resource was last modified.</rdfs:comment>
    <rdfs:domain rdf:resource="http://example.org/onto/class/google_beyondcorp_security_gateway"/>
    <rdfs:range rdf:resource="http://www.w3.org/2001/XMLSchema#string"/>
  </owl:DatatypeProperty>
  <owl:DatatypeProperty rdf:about="http://example.org/onto/prop/google_beyondcorp_security_gateway_region">
    <rdfs:label>region</rdfs:label>
    <rdfs:domain rdf:resource="http://example.org/onto/class/google_beyondcorp_security_gateway"/>
    <rdfs:range rdf:resource="http://www.w3.org/2001/XMLSchema#string"/>
  </owl:DatatypeProperty>
  <owl:DatatypeProperty rdf:about="http://example.org/onto/prop/google_beyondcorp_security_gateway_assigned_ips">
    <rdfs:label>assigned_ips</rdfs:label>
    <rdfs:comment>Output only. List of IP addresses assigned to the Cloud NAT.</rdfs:comment>
    <rdfs:domain rdf:resource="http://example.org/onto/class/google_beyondcorp_security_gateway"/>
    <rdfs:range rdf:resource="http://www.w3.org/2001/XMLSchema#string"/>
  </owl:DatatypeProperty>
  <owl:DatatypeProperty rdf:about="http://example.org/onto/prop/google_beyondcorp_security_gateway_allowed_client_headers">
    <rdfs:label>allowed_client_headers</rdfs:label>
    <rdfs:comment>The configuration for the proxy.</rdfs:comment>
    <rdfs:domain rdf:resource="http://example.org/onto/class/google_beyondcorp_security_gateway"/>
    <rdfs:range rdf:resource="http://www.w3.org/2001/XMLSchema#string"/>
  </owl:DatatypeProperty>
  <owl:DatatypeProperty rdf:about="http://example.org/onto/prop/google_beyondcorp_security_gateway_client_ip">
    <rdfs:label>client_ip</rdfs:label>
    <rdfs:comment>Client IP configuration. The client IP address is included if true.</rdfs:comment>
    <rdfs:domain rdf:resource="http://example.org/onto/class/google_beyondcorp_security_gateway"/>
    <rdfs:range rdf:resource="http://www.w3.org/2001/XMLSchema#string"/>
  </owl:DatatypeProperty>
  <owl:DatatypeProperty rdf:about="http://example.org/onto/prop/google_beyondcorp_security_gateway_gateway_identity">
    <rdfs:label>gateway_identity</rdfs:label>
    <rdfs:comment>Gateway identity configuration. Possible values: ["RESOURCE_NAME"]</rdfs:comment>
    <rdfs:domain rdf:resource="http://example.org/onto/class/google_beyondcorp_security_gateway"/>
    <rdfs:range rdf:resource="http://www.w3.org/2001/XMLSchema#string"/>
  </owl:DatatypeProperty>
  <owl:DatatypeProperty rdf:about="http://example.org/onto/prop/google_beyondcorp_security_gateway_metadata_headers">
    <rdfs:label>metadata_headers</rdfs:label>
    <rdfs:comment>Custom resource specific headers along with the values.
The names should conform to RFC 9110:
> Field names SHOULD constrain themselves to alphanumeric characters, "-",
  and ".", and SHOULD begin with a letter.
> Field values SHOULD contain only ASCII printable characters and tab.</rdfs:comment>
    <rdfs:domain rdf:resource="http://example.org/onto/class/google_beyondcorp_security_gateway"/>
    <rdfs:range rdf:resource="http://www.w3.org/2001/XMLSchema#string"/>
  </owl:DatatypeProperty>
  <owl:DatatypeProperty rdf:about="http://example.org/onto/prop/google_beyondcorp_security_gateway_output_type">
    <rdfs:label>output_type</rdfs:label>
    <rdfs:comment>Default output type for all enabled headers. Possible values: ["PROTOBUF", "JSON", "NONE"]</rdfs:comment>
    <rdfs:domain rdf:resource="http://example.org/onto/class/google_beyondcorp_security_gateway"/>
    <rdfs:range rdf:resource="http://www.w3.org/2001/XMLSchema#string"/>
  </owl:DatatypeProperty>
  <owl:DatatypeProperty rdf:about="http://example.org/onto/prop/google_beyondcorp_security_gateway_output_type">
    <rdfs:label>output_type</rdfs:label>
    <rdfs:comment>The output type of the delegated device info. Possible values: ["PROTOBUF", "JSON", "NONE"]</rdfs:comment>
    <rdfs:domain rdf:resource="http://example.org/onto/class/google_beyondcorp_security_gateway"/>
    <rdfs:range rdf:resource="http://www.w3.org/2001/XMLSchema#string"/>
  </owl:DatatypeProperty>
  <owl:DatatypeProperty rdf:about="http://example.org/onto/prop/google_beyondcorp_security_gateway_output_type">
    <rdfs:label>output_type</rdfs:label>
    <rdfs:comment>The output type of the delegated group info. Possible values: ["PROTOBUF", "JSON", "NONE"]</rdfs:comment>
    <rdfs:domain rdf:resource="http://example.org/onto/class/google_beyondcorp_security_gateway"/>
    <rdfs:range rdf:resource="http://www.w3.org/2001/XMLSchema#string"/>
  </owl:DatatypeProperty>
  <owl:DatatypeProperty rdf:about="http://example.org/onto/prop/google_beyondcorp_security_gateway_output_type">
    <rdfs:label>output_type</rdfs:label>
    <rdfs:comment>The output type of the delegated user info. Possible values: ["PROTOBUF", "JSON", "NONE"]</rdfs:comment>
    <rdfs:domain rdf:resource="http://example.org/onto/class/google_beyondcorp_security_gateway"/>
    <rdfs:range rdf:resource="http://www.w3.org/2001/XMLSchema#string"/>
  </owl:DatatypeProperty>
  <owl:DatatypeProperty rdf:about="http://example.org/onto/prop/google_beyondcorp_security_gateway_path">
    <rdfs:label>path</rdfs:label>
    <rdfs:comment>Contains uri path fragment where HTTP request is sent.</rdfs:comment>
    <rdfs:domain rdf:resource="http://example.org/onto/class/google_beyondcorp_security_gateway"/>
    <rdfs:range rdf:resource="http://www.w3.org/2001/XMLSchema#string"/>
  </owl:DatatypeProperty>
  <owl:DatatypeProperty rdf:about="http://example.org/onto/prop/google_beyondcorp_security_gateway_create">
    <rdfs:label>create</rdfs:label>
    <rdfs:domain rdf:resource="http://example.org/onto/class/google_beyondcorp_security_gateway"/>
    <rdfs:range rdf:resource="http://www.w3.org/2001/XMLSchema#string"/>
  </owl:DatatypeProperty>
  <owl:DatatypeProperty rdf:about="http://example.org/onto/prop/google_beyondcorp_security_gateway_delete">
    <rdfs:label>delete</rdfs:label>
    <rdfs:domain rdf:resource="http://example.org/onto/class/google_beyondcorp_security_gateway"/>
    <rdfs:range rdf:resource="http://www.w3.org/2001/XMLSchema#string"/>
  </owl:DatatypeProperty>
  <owl:DatatypeProperty rdf:about="http://example.org/onto/prop/google_beyondcorp_security_gateway_update">
    <rdfs:label>update</rdfs:label>
    <rdfs:domain rdf:resource="http://example.org/onto/class/google_beyondcorp_security_gateway"/>
    <rdfs:range rdf:resource="http://www.w3.org/2001/XMLSchema#string"/>
  </owl:DatatypeProperty>
</rdf:RDF>
