<?xml version="1.0" encoding="UTF-8"?>
<rdf:RDF
  xmlns:rdf="http://www.w3.org/1999/02/22-rdf-syntax-ns#"
  xmlns:rdfs="http://www.w3.org/2000/01/rdf-schema#"
  xmlns:owl="http://www.w3.org/2002/07/owl#"
  xmlns:xsd="http://www.w3.org/2001/XMLSchema#"
  xml:base="http://example.org/onto/">
  <owl:Class rdf:about="http://example.org/onto/class/google_memorystore_instance">
    <rdfs:label>google_memorystore_instance</rdfs:label>
    <rdfs:comment>#
#     ***     AUTO GENERATED CODE    ***    Type: MMv1     ***
#
# ----------------------------------------------------------------------------
#
#     This code is generated by Magic Modules using the following:
#
#     Configuration: https:#github.com/GoogleCloudPlatform/magic-modules/tree/main/mmv1/products/memorystore/Instance.yaml
#     Template:      https:#github.com/GoogleCloudPlatform/magic-modules/tree/main/mmv1/templates/terraform/resource.html.markdown.tmpl
#
#     DO NOT EDIT this file directly. Any changes made to this file will be
#     overwritten during the next generation cycle.
#
# ----------------------------------------------------------------------------
subcategory: "Memorystore"
description: |-
  A Google Cloud Memorystore instance.
---</rdfs:comment>
  </owl:Class>
  <owl:DatatypeProperty rdf:about="http://example.org/onto/prop/google_memorystore_instance_authorization_mode">
    <rdfs:label>authorization_mode</rdfs:label>
    <rdfs:comment>Optional. Immutable. Authorization mode of the instance. Possible values:
 AUTH_DISABLED
IAM_AUTH</rdfs:comment>
    <rdfs:domain rdf:resource="http://example.org/onto/class/google_memorystore_instance"/>
    <rdfs:range rdf:resource="http://www.w3.org/2001/XMLSchema#string"/>
  </owl:DatatypeProperty>
  <owl:DatatypeProperty rdf:about="http://example.org/onto/prop/google_memorystore_instance_backup_collection">
    <rdfs:label>backup_collection</rdfs:label>
    <rdfs:comment>The backup collection full resource name.
Example: projects/{project}/locations/{location}/backupCollections/{collection}</rdfs:comment>
    <rdfs:domain rdf:resource="http://example.org/onto/class/google_memorystore_instance"/>
    <rdfs:range rdf:resource="http://www.w3.org/2001/XMLSchema#string"/>
  </owl:DatatypeProperty>
  <owl:DatatypeProperty rdf:about="http://example.org/onto/prop/google_memorystore_instance_create_time">
    <rdfs:label>create_time</rdfs:label>
    <rdfs:comment>Output only. Creation timestamp of the instance.</rdfs:comment>
    <rdfs:domain rdf:resource="http://example.org/onto/class/google_memorystore_instance"/>
    <rdfs:range rdf:resource="http://www.w3.org/2001/XMLSchema#string"/>
  </owl:DatatypeProperty>
  <owl:DatatypeProperty rdf:about="http://example.org/onto/prop/google_memorystore_instance_deletion_protection_enabled">
    <rdfs:label>deletion_protection_enabled</rdfs:label>
    <rdfs:comment>Optional. If set to true deletion of the instance will fail.</rdfs:comment>
    <rdfs:domain rdf:resource="http://example.org/onto/class/google_memorystore_instance"/>
    <rdfs:range rdf:resource="http://www.w3.org/2001/XMLSchema#string"/>
  </owl:DatatypeProperty>
  <owl:DatatypeProperty rdf:about="http://example.org/onto/prop/google_memorystore_instance_discovery_endpoints">
    <rdfs:label>discovery_endpoints</rdfs:label>
    <rdfs:comment>Deprecated. Output only. Endpoints clients can connect to the instance through.</rdfs:comment>
    <rdfs:domain rdf:resource="http://example.org/onto/class/google_memorystore_instance"/>
    <rdfs:range rdf:resource="http://www.w3.org/2001/XMLSchema#string"/>
  </owl:DatatypeProperty>
  <owl:DatatypeProperty rdf:about="http://example.org/onto/prop/google_memorystore_instance_effective_labels">
    <rdfs:label>effective_labels</rdfs:label>
    <rdfs:comment>All of labels (key/value pairs) present on the resource in GCP, including the labels configured through Terraform, other clients and services.</rdfs:comment>
    <rdfs:domain rdf:resource="http://example.org/onto/class/google_memorystore_instance"/>
    <rdfs:range rdf:resource="http://www.w3.org/2001/XMLSchema#string"/>
  </owl:DatatypeProperty>
  <owl:DatatypeProperty rdf:about="http://example.org/onto/prop/google_memorystore_instance_endpoints">
    <rdfs:label>endpoints</rdfs:label>
    <rdfs:comment>Endpoints for the instance.</rdfs:comment>
    <rdfs:domain rdf:resource="http://example.org/onto/class/google_memorystore_instance"/>
    <rdfs:range rdf:resource="http://www.w3.org/2001/XMLSchema#string"/>
  </owl:DatatypeProperty>
  <owl:DatatypeProperty rdf:about="http://example.org/onto/prop/google_memorystore_instance_engine_configs">
    <rdfs:label>engine_configs</rdfs:label>
    <rdfs:comment>Optional. User-provided engine configurations for the instance.</rdfs:comment>
    <rdfs:domain rdf:resource="http://example.org/onto/class/google_memorystore_instance"/>
    <rdfs:range rdf:resource="http://www.w3.org/2001/XMLSchema#string"/>
  </owl:DatatypeProperty>
  <owl:DatatypeProperty rdf:about="http://example.org/onto/prop/google_memorystore_instance_engine_version">
    <rdfs:label>engine_version</rdfs:label>
    <rdfs:comment>Optional. Engine version of the instance.</rdfs:comment>
    <rdfs:domain rdf:resource="http://example.org/onto/class/google_memorystore_instance"/>
    <rdfs:range rdf:resource="http://www.w3.org/2001/XMLSchema#string"/>
  </owl:DatatypeProperty>
  <owl:DatatypeProperty rdf:about="http://example.org/onto/prop/google_memorystore_instance_id">
    <rdfs:label>id</rdfs:label>
    <rdfs:domain rdf:resource="http://example.org/onto/class/google_memorystore_instance"/>
    <rdfs:range rdf:resource="http://www.w3.org/2001/XMLSchema#string"/>
  </owl:DatatypeProperty>
  <owl:DatatypeProperty rdf:about="http://example.org/onto/prop/google_memorystore_instance_instance_id">
    <rdfs:label>instance_id</rdfs:label>
    <rdfs:comment>Required. The ID to use for the instance, which will become the final component of
the instance's resource name.

This value is subject to the following restrictions:

* Must be 4-63 characters in length
* Must begin with a letter or digit
* Must contain only lowercase letters, digits, and hyphens
* Must not end with a hyphen
* Must be unique within a location</rdfs:comment>
    <rdfs:domain rdf:resource="http://example.org/onto/class/google_memorystore_instance"/>
    <rdfs:range rdf:resource="http://www.w3.org/2001/XMLSchema#string"/>
  </owl:DatatypeProperty>
  <owl:DatatypeProperty rdf:about="http://example.org/onto/prop/google_memorystore_instance_kms_key">
    <rdfs:label>kms_key</rdfs:label>
    <rdfs:comment>The KMS key used to encrypt the at-rest data of the cluster</rdfs:comment>
    <rdfs:domain rdf:resource="http://example.org/onto/class/google_memorystore_instance"/>
    <rdfs:range rdf:resource="http://www.w3.org/2001/XMLSchema#string"/>
  </owl:DatatypeProperty>
  <owl:DatatypeProperty rdf:about="http://example.org/onto/prop/google_memorystore_instance_labels">
    <rdfs:label>labels</rdfs:label>
    <rdfs:comment>Optional. Labels to represent user-provided metadata. 

**Note**: This field is non-authoritative, and will only manage the labels present in your configuration.
Please refer to the field 'effective_labels' for all of the labels present on the resource.</rdfs:comment>
    <rdfs:domain rdf:resource="http://example.org/onto/class/google_memorystore_instance"/>
    <rdfs:range rdf:resource="http://www.w3.org/2001/XMLSchema#string"/>
  </owl:DatatypeProperty>
  <owl:DatatypeProperty rdf:about="http://example.org/onto/prop/google_memorystore_instance_location">
    <rdfs:label>location</rdfs:label>
    <rdfs:comment>Resource ID segment making up resource 'name'. It identifies the resource within its parent collection as described in https://google.aip.dev/122. See documentation for resource type 'memorystore.googleapis.com/CertificateAuthority'.</rdfs:comment>
    <rdfs:domain rdf:resource="http://example.org/onto/class/google_memorystore_instance"/>
    <rdfs:range rdf:resource="http://www.w3.org/2001/XMLSchema#string"/>
  </owl:DatatypeProperty>
  <owl:DatatypeProperty rdf:about="http://example.org/onto/prop/google_memorystore_instance_maintenance_schedule">
    <rdfs:label>maintenance_schedule</rdfs:label>
    <rdfs:comment>Upcoming maintenance schedule.</rdfs:comment>
    <rdfs:domain rdf:resource="http://example.org/onto/class/google_memorystore_instance"/>
    <rdfs:range rdf:resource="http://www.w3.org/2001/XMLSchema#string"/>
  </owl:DatatypeProperty>
  <owl:DatatypeProperty rdf:about="http://example.org/onto/prop/google_memorystore_instance_managed_server_ca">
    <rdfs:label>managed_server_ca</rdfs:label>
    <rdfs:comment>Instance's Certificate Authority. This field will only be populated if instance's transit_encryption_mode is SERVER_AUTHENTICATION</rdfs:comment>
    <rdfs:domain rdf:resource="http://example.org/onto/class/google_memorystore_instance"/>
    <rdfs:range rdf:resource="http://www.w3.org/2001/XMLSchema#string"/>
  </owl:DatatypeProperty>
  <owl:DatatypeProperty rdf:about="http://example.org/onto/prop/google_memorystore_instance_mode">
    <rdfs:label>mode</rdfs:label>
    <rdfs:comment>Optional. cluster or cluster-disabled. 
 Possible values:
 CLUSTER
 CLUSTER_DISABLED Possible values: ["CLUSTER", "CLUSTER_DISABLED"]</rdfs:comment>
    <rdfs:domain rdf:resource="http://example.org/onto/class/google_memorystore_instance"/>
    <rdfs:range rdf:resource="http://www.w3.org/2001/XMLSchema#string"/>
  </owl:DatatypeProperty>
  <owl:DatatypeProperty rdf:about="http://example.org/onto/prop/google_memorystore_instance_name">
    <rdfs:label>name</rdfs:label>
    <rdfs:comment>Identifier. Unique name of the instance.
Format: projects/{project}/locations/{location}/instances/{instance}</rdfs:comment>
    <rdfs:domain rdf:resource="http://example.org/onto/class/google_memorystore_instance"/>
    <rdfs:range rdf:resource="http://www.w3.org/2001/XMLSchema#string"/>
  </owl:DatatypeProperty>
  <owl:DatatypeProperty rdf:about="http://example.org/onto/prop/google_memorystore_instance_node_config">
    <rdfs:label>node_config</rdfs:label>
    <rdfs:comment>Represents configuration for nodes of the instance.</rdfs:comment>
    <rdfs:domain rdf:resource="http://example.org/onto/class/google_memorystore_instance"/>
    <rdfs:range rdf:resource="http://www.w3.org/2001/XMLSchema#string"/>
  </owl:DatatypeProperty>
  <owl:DatatypeProperty rdf:about="http://example.org/onto/prop/google_memorystore_instance_node_type">
    <rdfs:label>node_type</rdfs:label>
    <rdfs:comment>Optional. Machine type for individual nodes of the instance. 
 Possible values:
 SHARED_CORE_NANO
HIGHMEM_MEDIUM
HIGHMEM_XLARGE
STANDARD_SMALL</rdfs:comment>
    <rdfs:domain rdf:resource="http://example.org/onto/class/google_memorystore_instance"/>
    <rdfs:range rdf:resource="http://www.w3.org/2001/XMLSchema#string"/>
  </owl:DatatypeProperty>
  <owl:DatatypeProperty rdf:about="http://example.org/onto/prop/google_memorystore_instance_project">
    <rdfs:label>project</rdfs:label>
    <rdfs:domain rdf:resource="http://example.org/onto/class/google_memorystore_instance"/>
    <rdfs:range rdf:resource="http://www.w3.org/2001/XMLSchema#string"/>
  </owl:DatatypeProperty>
  <owl:DatatypeProperty rdf:about="http://example.org/onto/prop/google_memorystore_instance_psc_attachment_details">
    <rdfs:label>psc_attachment_details</rdfs:label>
    <rdfs:comment>Configuration of a service attachment of the cluster, for creating PSC connections.</rdfs:comment>
    <rdfs:domain rdf:resource="http://example.org/onto/class/google_memorystore_instance"/>
    <rdfs:range rdf:resource="http://www.w3.org/2001/XMLSchema#string"/>
  </owl:DatatypeProperty>
  <owl:DatatypeProperty rdf:about="http://example.org/onto/prop/google_memorystore_instance_psc_auto_connections">
    <rdfs:label>psc_auto_connections</rdfs:label>
    <rdfs:comment>Output only. User inputs and resource details of the auto-created PSC connections.</rdfs:comment>
    <rdfs:domain rdf:resource="http://example.org/onto/class/google_memorystore_instance"/>
    <rdfs:range rdf:resource="http://www.w3.org/2001/XMLSchema#string"/>
  </owl:DatatypeProperty>
  <owl:DatatypeProperty rdf:about="http://example.org/onto/prop/google_memorystore_instance_replica_count">
    <rdfs:label>replica_count</rdfs:label>
    <rdfs:comment>Optional. Number of replica nodes per shard. If omitted the default is 0 replicas.</rdfs:comment>
    <rdfs:domain rdf:resource="http://example.org/onto/class/google_memorystore_instance"/>
    <rdfs:range rdf:resource="http://www.w3.org/2001/XMLSchema#string"/>
  </owl:DatatypeProperty>
  <owl:DatatypeProperty rdf:about="http://example.org/onto/prop/google_memorystore_instance_shard_count">
    <rdfs:label>shard_count</rdfs:label>
    <rdfs:comment>Required. Number of shards for the instance.</rdfs:comment>
    <rdfs:domain rdf:resource="http://example.org/onto/class/google_memorystore_instance"/>
    <rdfs:range rdf:resource="http://www.w3.org/2001/XMLSchema#string"/>
  </owl:DatatypeProperty>
  <owl:DatatypeProperty rdf:about="http://example.org/onto/prop/google_memorystore_instance_state">
    <rdfs:label>state</rdfs:label>
    <rdfs:comment>Output only. Current state of the instance. 
 Possible values:
 CREATING
ACTIVE
UPDATING
DELETING</rdfs:comment>
    <rdfs:domain rdf:resource="http://example.org/onto/class/google_memorystore_instance"/>
    <rdfs:range rdf:resource="http://www.w3.org/2001/XMLSchema#string"/>
  </owl:DatatypeProperty>
  <owl:DatatypeProperty rdf:about="http://example.org/onto/prop/google_memorystore_instance_state_info">
    <rdfs:label>state_info</rdfs:label>
    <rdfs:comment>Additional information about the state of the instance.</rdfs:comment>
    <rdfs:domain rdf:resource="http://example.org/onto/class/google_memorystore_instance"/>
    <rdfs:range rdf:resource="http://www.w3.org/2001/XMLSchema#string"/>
  </owl:DatatypeProperty>
  <owl:DatatypeProperty rdf:about="http://example.org/onto/prop/google_memorystore_instance_terraform_labels">
    <rdfs:label>terraform_labels</rdfs:label>
    <rdfs:comment>The combination of labels configured directly on the resource
 and default labels configured on the provider.</rdfs:comment>
    <rdfs:domain rdf:resource="http://example.org/onto/class/google_memorystore_instance"/>
    <rdfs:range rdf:resource="http://www.w3.org/2001/XMLSchema#string"/>
  </owl:DatatypeProperty>
  <owl:DatatypeProperty rdf:about="http://example.org/onto/prop/google_memorystore_instance_transit_encryption_mode">
    <rdfs:label>transit_encryption_mode</rdfs:label>
    <rdfs:comment>Optional. Immutable. In-transit encryption mode of the instance. 
 Possible values:
 TRANSIT_ENCRYPTION_DISABLED
SERVER_AUTHENTICATION</rdfs:comment>
    <rdfs:domain rdf:resource="http://example.org/onto/class/google_memorystore_instance"/>
    <rdfs:range rdf:resource="http://www.w3.org/2001/XMLSchema#string"/>
  </owl:DatatypeProperty>
  <owl:DatatypeProperty rdf:about="http://example.org/onto/prop/google_memorystore_instance_uid">
    <rdfs:label>uid</rdfs:label>
    <rdfs:comment>Output only. System assigned, unique identifier for the instance.</rdfs:comment>
    <rdfs:domain rdf:resource="http://example.org/onto/class/google_memorystore_instance"/>
    <rdfs:range rdf:resource="http://www.w3.org/2001/XMLSchema#string"/>
  </owl:DatatypeProperty>
  <owl:DatatypeProperty rdf:about="http://example.org/onto/prop/google_memorystore_instance_update_time">
    <rdfs:label>update_time</rdfs:label>
    <rdfs:comment>Output only. Latest update timestamp of the instance.</rdfs:comment>
    <rdfs:domain rdf:resource="http://example.org/onto/class/google_memorystore_instance"/>
    <rdfs:range rdf:resource="http://www.w3.org/2001/XMLSchema#string"/>
  </owl:DatatypeProperty>
  <owl:DatatypeProperty rdf:about="http://example.org/onto/prop/google_memorystore_instance_retention">
    <rdfs:label>retention</rdfs:label>
    <rdfs:comment>How long to keep automated backups before the backups are deleted.
The value should be between 1 day and 365 days. If not specified, the default value is 35 days.
A duration in seconds with up to nine fractional digits, ending with 's'. Example: "3.5s". The default_value is "3024000s"</rdfs:comment>
    <rdfs:domain rdf:resource="http://example.org/onto/class/google_memorystore_instance"/>
    <rdfs:range rdf:resource="http://www.w3.org/2001/XMLSchema#string"/>
  </owl:DatatypeProperty>
  <owl:DatatypeProperty rdf:about="http://example.org/onto/prop/google_memorystore_instance_hours">
    <rdfs:label>hours</rdfs:label>
    <rdfs:comment>Hours of a day in 24 hour format. Must be greater than or equal to 0 and typically must be less than or equal to 23.
An API may choose to allow the value "24:00:00" for scenarios like business closing time.</rdfs:comment>
    <rdfs:domain rdf:resource="http://example.org/onto/class/google_memorystore_instance"/>
    <rdfs:range rdf:resource="http://www.w3.org/2001/XMLSchema#string"/>
  </owl:DatatypeProperty>
  <owl:DatatypeProperty rdf:about="http://example.org/onto/prop/google_memorystore_instance_instance_role">
    <rdfs:label>instance_role</rdfs:label>
    <rdfs:comment>The instance role supports the following values:
1. 'INSTANCE_ROLE_UNSPECIFIED': This is an independent instance that has never participated in cross instance replication. It allows both reads and writes.
2. 'NONE': This is an independent instance that previously participated in cross instance replication(either as a 'PRIMARY' or 'SECONDARY' cluster). It allows both reads and writes.
3. 'PRIMARY': This instance serves as the replication source for secondary instance that are replicating from it. Any data written to it is automatically replicated to its secondary clusters. It allows both reads and writes.
4. 'SECONDARY': This instance replicates data from the primary instance. It allows only reads. Possible values: ["INSTANCE_ROLE_UNSPECIFIED", "NONE", "PRIMARY", "SECONDARY"]</rdfs:comment>
    <rdfs:domain rdf:resource="http://example.org/onto/class/google_memorystore_instance"/>
    <rdfs:range rdf:resource="http://www.w3.org/2001/XMLSchema#string"/>
  </owl:DatatypeProperty>
  <owl:DatatypeProperty rdf:about="http://example.org/onto/prop/google_memorystore_instance_membership">
    <rdfs:label>membership</rdfs:label>
    <rdfs:comment>An output only view of all the member instance participating in cross instance replication. This field is populated for all the member clusters irrespective of their cluster role.</rdfs:comment>
    <rdfs:domain rdf:resource="http://example.org/onto/class/google_memorystore_instance"/>
    <rdfs:range rdf:resource="http://www.w3.org/2001/XMLSchema#string"/>
  </owl:DatatypeProperty>
  <owl:DatatypeProperty rdf:about="http://example.org/onto/prop/google_memorystore_instance_update_time">
    <rdfs:label>update_time</rdfs:label>
    <rdfs:comment>The last time cross instance replication config was updated.</rdfs:comment>
    <rdfs:domain rdf:resource="http://example.org/onto/class/google_memorystore_instance"/>
    <rdfs:range rdf:resource="http://www.w3.org/2001/XMLSchema#string"/>
  </owl:DatatypeProperty>
  <owl:DatatypeProperty rdf:about="http://example.org/onto/prop/google_memorystore_instance_instance">
    <rdfs:label>instance</rdfs:label>
    <rdfs:comment>The full resource path of the primary instance in the format: projects/{project}/locations/{region}/instances/{instance-id}</rdfs:comment>
    <rdfs:domain rdf:resource="http://example.org/onto/class/google_memorystore_instance"/>
    <rdfs:range rdf:resource="http://www.w3.org/2001/XMLSchema#string"/>
  </owl:DatatypeProperty>
  <owl:DatatypeProperty rdf:about="http://example.org/onto/prop/google_memorystore_instance_uid">
    <rdfs:label>uid</rdfs:label>
    <rdfs:comment>The unique id of the primary instance.</rdfs:comment>
    <rdfs:domain rdf:resource="http://example.org/onto/class/google_memorystore_instance"/>
    <rdfs:range rdf:resource="http://www.w3.org/2001/XMLSchema#string"/>
  </owl:DatatypeProperty>
  <owl:DatatypeProperty rdf:about="http://example.org/onto/prop/google_memorystore_instance_instance">
    <rdfs:label>instance</rdfs:label>
    <rdfs:comment>The full resource path of the Nth instance in the format: projects/{project}/locations/{region}/instance/{instance-id}</rdfs:comment>
    <rdfs:domain rdf:resource="http://example.org/onto/class/google_memorystore_instance"/>
    <rdfs:range rdf:resource="http://www.w3.org/2001/XMLSchema#string"/>
  </owl:DatatypeProperty>
  <owl:DatatypeProperty rdf:about="http://example.org/onto/prop/google_memorystore_instance_uid">
    <rdfs:label>uid</rdfs:label>
    <rdfs:comment>The unique id of the Nth instance.</rdfs:comment>
    <rdfs:domain rdf:resource="http://example.org/onto/class/google_memorystore_instance"/>
    <rdfs:range rdf:resource="http://www.w3.org/2001/XMLSchema#string"/>
  </owl:DatatypeProperty>
  <owl:DatatypeProperty rdf:about="http://example.org/onto/prop/google_memorystore_instance_network">
    <rdfs:label>network</rdfs:label>
    <rdfs:comment>Required. The consumer network where the IP address resides, in the form of
projects/{project_id}/global/networks/{network_id}.</rdfs:comment>
    <rdfs:domain rdf:resource="http://example.org/onto/class/google_memorystore_instance"/>
    <rdfs:range rdf:resource="http://www.w3.org/2001/XMLSchema#string"/>
  </owl:DatatypeProperty>
  <owl:DatatypeProperty rdf:about="http://example.org/onto/prop/google_memorystore_instance_project_id">
    <rdfs:label>project_id</rdfs:label>
    <rdfs:comment>Required. The consumer project_id where the forwarding rule is created from.</rdfs:comment>
    <rdfs:domain rdf:resource="http://example.org/onto/class/google_memorystore_instance"/>
    <rdfs:range rdf:resource="http://www.w3.org/2001/XMLSchema#string"/>
  </owl:DatatypeProperty>
  <owl:DatatypeProperty rdf:about="http://example.org/onto/prop/google_memorystore_instance_network">
    <rdfs:label>network</rdfs:label>
    <rdfs:comment>Required. The consumer network where the IP address resides, in the form of
projects/{project_id}/global/networks/{network_id}.</rdfs:comment>
    <rdfs:domain rdf:resource="http://example.org/onto/class/google_memorystore_instance"/>
    <rdfs:range rdf:resource="http://www.w3.org/2001/XMLSchema#string"/>
  </owl:DatatypeProperty>
  <owl:DatatypeProperty rdf:about="http://example.org/onto/prop/google_memorystore_instance_project_id">
    <rdfs:label>project_id</rdfs:label>
    <rdfs:comment>Required. The consumer project_id where the forwarding rule is created from.</rdfs:comment>
    <rdfs:domain rdf:resource="http://example.org/onto/class/google_memorystore_instance"/>
    <rdfs:range rdf:resource="http://www.w3.org/2001/XMLSchema#string"/>
  </owl:DatatypeProperty>
  <owl:DatatypeProperty rdf:about="http://example.org/onto/prop/google_memorystore_instance_uris">
    <rdfs:label>uris</rdfs:label>
    <rdfs:comment>URIs of the GCS objects to import.
Example: gs://bucket1/object1, gs://bucket2/folder2/object2</rdfs:comment>
    <rdfs:domain rdf:resource="http://example.org/onto/class/google_memorystore_instance"/>
    <rdfs:range rdf:resource="http://www.w3.org/2001/XMLSchema#string"/>
  </owl:DatatypeProperty>
  <owl:DatatypeProperty rdf:about="http://example.org/onto/prop/google_memorystore_instance_create_time">
    <rdfs:label>create_time</rdfs:label>
    <rdfs:comment>The time when the policy was created.
A timestamp in RFC3339 UTC "Zulu" format, with nanosecond
resolution and up to nine fractional digits.</rdfs:comment>
    <rdfs:domain rdf:resource="http://example.org/onto/class/google_memorystore_instance"/>
    <rdfs:range rdf:resource="http://www.w3.org/2001/XMLSchema#string"/>
  </owl:DatatypeProperty>
  <owl:DatatypeProperty rdf:about="http://example.org/onto/prop/google_memorystore_instance_update_time">
    <rdfs:label>update_time</rdfs:label>
    <rdfs:comment>The time when the policy was last updated.
A timestamp in RFC3339 UTC "Zulu" format, with nanosecond
resolution and up to nine fractional digits.</rdfs:comment>
    <rdfs:domain rdf:resource="http://example.org/onto/class/google_memorystore_instance"/>
    <rdfs:range rdf:resource="http://www.w3.org/2001/XMLSchema#string"/>
  </owl:DatatypeProperty>
  <owl:DatatypeProperty rdf:about="http://example.org/onto/prop/google_memorystore_instance_day">
    <rdfs:label>day</rdfs:label>
    <rdfs:comment>The day of week that maintenance updates occur.

- DAY_OF_WEEK_UNSPECIFIED: The day of the week is unspecified.
- MONDAY: Monday
- TUESDAY: Tuesday
- WEDNESDAY: Wednesday
- THURSDAY: Thursday
- FRIDAY: Friday
- SATURDAY: Saturday
- SUNDAY: Sunday Possible values: ["DAY_OF_WEEK_UNSPECIFIED", "MONDAY", "TUESDAY", "WEDNESDAY", "THURSDAY", "FRIDAY", "SATURDAY", "SUNDAY"]</rdfs:comment>
    <rdfs:domain rdf:resource="http://example.org/onto/class/google_memorystore_instance"/>
    <rdfs:range rdf:resource="http://www.w3.org/2001/XMLSchema#string"/>
  </owl:DatatypeProperty>
  <owl:DatatypeProperty rdf:about="http://example.org/onto/prop/google_memorystore_instance_duration">
    <rdfs:label>duration</rdfs:label>
    <rdfs:comment>Duration of the maintenance window.
The current window is fixed at 1 hour.
A duration in seconds with up to nine fractional digits,
terminated by 's'. Example: "3.5s".</rdfs:comment>
    <rdfs:domain rdf:resource="http://example.org/onto/class/google_memorystore_instance"/>
    <rdfs:range rdf:resource="http://www.w3.org/2001/XMLSchema#string"/>
  </owl:DatatypeProperty>
  <owl:DatatypeProperty rdf:about="http://example.org/onto/prop/google_memorystore_instance_hours">
    <rdfs:label>hours</rdfs:label>
    <rdfs:comment>Hours of day in 24 hour format. Should be from 0 to 23.
An API may choose to allow the value "24:00:00" for scenarios like business closing time.</rdfs:comment>
    <rdfs:domain rdf:resource="http://example.org/onto/class/google_memorystore_instance"/>
    <rdfs:range rdf:resource="http://www.w3.org/2001/XMLSchema#string"/>
  </owl:DatatypeProperty>
  <owl:DatatypeProperty rdf:about="http://example.org/onto/prop/google_memorystore_instance_minutes">
    <rdfs:label>minutes</rdfs:label>
    <rdfs:comment>Minutes of hour of day. Must be from 0 to 59.</rdfs:comment>
    <rdfs:domain rdf:resource="http://example.org/onto/class/google_memorystore_instance"/>
    <rdfs:range rdf:resource="http://www.w3.org/2001/XMLSchema#string"/>
  </owl:DatatypeProperty>
  <owl:DatatypeProperty rdf:about="http://example.org/onto/prop/google_memorystore_instance_nanos">
    <rdfs:label>nanos</rdfs:label>
    <rdfs:comment>Fractions of seconds in nanoseconds. Must be from 0 to 999,999,999.</rdfs:comment>
    <rdfs:domain rdf:resource="http://example.org/onto/class/google_memorystore_instance"/>
    <rdfs:range rdf:resource="http://www.w3.org/2001/XMLSchema#string"/>
  </owl:DatatypeProperty>
  <owl:DatatypeProperty rdf:about="http://example.org/onto/prop/google_memorystore_instance_seconds">
    <rdfs:label>seconds</rdfs:label>
    <rdfs:comment>Seconds of minutes of the time. Must normally be from 0 to 59.
An API may allow the value 60 if it allows leap-seconds.</rdfs:comment>
    <rdfs:domain rdf:resource="http://example.org/onto/class/google_memorystore_instance"/>
    <rdfs:range rdf:resource="http://www.w3.org/2001/XMLSchema#string"/>
  </owl:DatatypeProperty>
  <owl:DatatypeProperty rdf:about="http://example.org/onto/prop/google_memorystore_instance_backup">
    <rdfs:label>backup</rdfs:label>
    <rdfs:comment>Example: 'projects/{project}/locations/{location}/backupCollections/{collection}/backups/{backup}'.</rdfs:comment>
    <rdfs:domain rdf:resource="http://example.org/onto/class/google_memorystore_instance"/>
    <rdfs:range rdf:resource="http://www.w3.org/2001/XMLSchema#string"/>
  </owl:DatatypeProperty>
  <owl:DatatypeProperty rdf:about="http://example.org/onto/prop/google_memorystore_instance_mode">
    <rdfs:label>mode</rdfs:label>
    <rdfs:comment>Optional. Current persistence mode. 
 Possible values:
DISABLED
RDB
AOF Possible values: ["DISABLED", "RDB", "AOF"]</rdfs:comment>
    <rdfs:domain rdf:resource="http://example.org/onto/class/google_memorystore_instance"/>
    <rdfs:range rdf:resource="http://www.w3.org/2001/XMLSchema#string"/>
  </owl:DatatypeProperty>
  <owl:DatatypeProperty rdf:about="http://example.org/onto/prop/google_memorystore_instance_append_fsync">
    <rdfs:label>append_fsync</rdfs:label>
    <rdfs:comment>Optional. The fsync mode. 
 Possible values:
 NEVER
EVERY_SEC
ALWAYS</rdfs:comment>
    <rdfs:domain rdf:resource="http://example.org/onto/class/google_memorystore_instance"/>
    <rdfs:range rdf:resource="http://www.w3.org/2001/XMLSchema#string"/>
  </owl:DatatypeProperty>
  <owl:DatatypeProperty rdf:about="http://example.org/onto/prop/google_memorystore_instance_rdb_snapshot_period">
    <rdfs:label>rdb_snapshot_period</rdfs:label>
    <rdfs:comment>Optional. Period between RDB snapshots. 
 Possible values:
 ONE_HOUR
SIX_HOURS
TWELVE_HOURS
TWENTY_FOUR_HOURS</rdfs:comment>
    <rdfs:domain rdf:resource="http://example.org/onto/class/google_memorystore_instance"/>
    <rdfs:range rdf:resource="http://www.w3.org/2001/XMLSchema#string"/>
  </owl:DatatypeProperty>
  <owl:DatatypeProperty rdf:about="http://example.org/onto/prop/google_memorystore_instance_rdb_snapshot_start_time">
    <rdfs:label>rdb_snapshot_start_time</rdfs:label>
    <rdfs:comment>Optional. Time that the first snapshot was/will be attempted, and to which future
snapshots will be aligned. If not provided, the current time will be
used.</rdfs:comment>
    <rdfs:domain rdf:resource="http://example.org/onto/class/google_memorystore_instance"/>
    <rdfs:range rdf:resource="http://www.w3.org/2001/XMLSchema#string"/>
  </owl:DatatypeProperty>
  <owl:DatatypeProperty rdf:about="http://example.org/onto/prop/google_memorystore_instance_create">
    <rdfs:label>create</rdfs:label>
    <rdfs:domain rdf:resource="http://example.org/onto/class/google_memorystore_instance"/>
    <rdfs:range rdf:resource="http://www.w3.org/2001/XMLSchema#string"/>
  </owl:DatatypeProperty>
  <owl:DatatypeProperty rdf:about="http://example.org/onto/prop/google_memorystore_instance_delete">
    <rdfs:label>delete</rdfs:label>
    <rdfs:domain rdf:resource="http://example.org/onto/class/google_memorystore_instance"/>
    <rdfs:range rdf:resource="http://www.w3.org/2001/XMLSchema#string"/>
  </owl:DatatypeProperty>
  <owl:DatatypeProperty rdf:about="http://example.org/onto/prop/google_memorystore_instance_update">
    <rdfs:label>update</rdfs:label>
    <rdfs:domain rdf:resource="http://example.org/onto/class/google_memorystore_instance"/>
    <rdfs:range rdf:resource="http://www.w3.org/2001/XMLSchema#string"/>
  </owl:DatatypeProperty>
  <owl:DatatypeProperty rdf:about="http://example.org/onto/prop/google_memorystore_instance_mode">
    <rdfs:label>mode</rdfs:label>
    <rdfs:comment>Optional. Current zone distribution mode. Defaults to MULTI_ZONE. 
 Possible values:
 MULTI_ZONE
SINGLE_ZONE Possible values: ["MULTI_ZONE", "SINGLE_ZONE"]</rdfs:comment>
    <rdfs:domain rdf:resource="http://example.org/onto/class/google_memorystore_instance"/>
    <rdfs:range rdf:resource="http://www.w3.org/2001/XMLSchema#string"/>
  </owl:DatatypeProperty>
  <owl:DatatypeProperty rdf:about="http://example.org/onto/prop/google_memorystore_instance_zone">
    <rdfs:label>zone</rdfs:label>
    <rdfs:comment>Optional. Defines zone where all resources will be allocated with SINGLE_ZONE mode.
Ignored for MULTI_ZONE mode.</rdfs:comment>
    <rdfs:domain rdf:resource="http://example.org/onto/class/google_memorystore_instance"/>
    <rdfs:range rdf:resource="http://www.w3.org/2001/XMLSchema#string"/>
  </owl:DatatypeProperty>
</rdf:RDF>
