<?xml version="1.0" encoding="UTF-8"?>
<rdf:RDF
  xmlns:rdf="http://www.w3.org/1999/02/22-rdf-syntax-ns#"
  xmlns:rdfs="http://www.w3.org/2000/01/rdf-schema#"
  xmlns:owl="http://www.w3.org/2002/07/owl#"
  xmlns:xsd="http://www.w3.org/2001/XMLSchema#"
  xml:base="http://example.org/onto/">
  <owl:Class rdf:about="http://example.org/onto/class/google_monitoring_monitored_project">
    <rdfs:label>google_monitoring_monitored_project</rdfs:label>
    <rdfs:comment>#
#     ***     AUTO GENERATED CODE    ***    Type: MMv1     ***
#
# ----------------------------------------------------------------------------
#
#     This code is generated by Magic Modules using the following:
#
#     Configuration: https:#github.com/GoogleCloudPlatform/magic-modules/tree/main/mmv1/products/monitoring/MonitoredProject.yaml
#     Template:      https:#github.com/GoogleCloudPlatform/magic-modules/tree/main/mmv1/templates/terraform/resource.html.markdown.tmpl
#
#     DO NOT EDIT this file directly. Any changes made to this file will be
#     overwritten during the next generation cycle.
#
# ----------------------------------------------------------------------------
subcategory: "Cloud (Stackdriver) Monitoring"
description: |-
  A [project being monitored](https://cloud.
---</rdfs:comment>
  </owl:Class>
  <owl:DatatypeProperty rdf:about="http://example.org/onto/prop/google_monitoring_monitored_project_create_time">
    <rdfs:label>create_time</rdfs:label>
    <rdfs:comment>Output only. The time when this 'MonitoredProject' was created.</rdfs:comment>
    <rdfs:domain rdf:resource="http://example.org/onto/class/google_monitoring_monitored_project"/>
    <rdfs:range rdf:resource="http://www.w3.org/2001/XMLSchema#string"/>
  </owl:DatatypeProperty>
  <owl:DatatypeProperty rdf:about="http://example.org/onto/prop/google_monitoring_monitored_project_id">
    <rdfs:label>id</rdfs:label>
    <rdfs:domain rdf:resource="http://example.org/onto/class/google_monitoring_monitored_project"/>
    <rdfs:range rdf:resource="http://www.w3.org/2001/XMLSchema#string"/>
  </owl:DatatypeProperty>
  <owl:DatatypeProperty rdf:about="http://example.org/onto/prop/google_monitoring_monitored_project_metrics_scope">
    <rdfs:label>metrics_scope</rdfs:label>
    <rdfs:comment>Required. The resource name of the existing Metrics Scope that will monitor this project. Example: locations/global/metricsScopes/{SCOPING_PROJECT_ID_OR_NUMBER}</rdfs:comment>
    <rdfs:domain rdf:resource="http://example.org/onto/class/google_monitoring_monitored_project"/>
    <rdfs:range rdf:resource="http://www.w3.org/2001/XMLSchema#string"/>
  </owl:DatatypeProperty>
  <owl:DatatypeProperty rdf:about="http://example.org/onto/prop/google_monitoring_monitored_project_name">
    <rdfs:label>name</rdfs:label>
    <rdfs:comment>Immutable. The resource name of the 'MonitoredProject'. On input, the resource name includes the scoping project ID and monitored project ID. On output, it contains the equivalent project numbers. Example: 'locations/global/metricsScopes/{SCOPING_PROJECT_ID_OR_NUMBER}/projects/{MONITORED_PROJECT_ID_OR_NUMBER}'</rdfs:comment>
    <rdfs:domain rdf:resource="http://example.org/onto/class/google_monitoring_monitored_project"/>
    <rdfs:range rdf:resource="http://www.w3.org/2001/XMLSchema#string"/>
  </owl:DatatypeProperty>
  <owl:DatatypeProperty rdf:about="http://example.org/onto/prop/google_monitoring_monitored_project_create">
    <rdfs:label>create</rdfs:label>
    <rdfs:domain rdf:resource="http://example.org/onto/class/google_monitoring_monitored_project"/>
    <rdfs:range rdf:resource="http://www.w3.org/2001/XMLSchema#string"/>
  </owl:DatatypeProperty>
  <owl:DatatypeProperty rdf:about="http://example.org/onto/prop/google_monitoring_monitored_project_delete">
    <rdfs:label>delete</rdfs:label>
    <rdfs:domain rdf:resource="http://example.org/onto/class/google_monitoring_monitored_project"/>
    <rdfs:range rdf:resource="http://www.w3.org/2001/XMLSchema#string"/>
  </owl:DatatypeProperty>
</rdf:RDF>
