<?xml version="1.0" encoding="UTF-8"?>
<rdf:RDF
  xmlns:rdf="http://www.w3.org/1999/02/22-rdf-syntax-ns#"
  xmlns:rdfs="http://www.w3.org/2000/01/rdf-schema#"
  xmlns:owl="http://www.w3.org/2002/07/owl#"
  xmlns:xsd="http://www.w3.org/2001/XMLSchema#"
  xml:base="http://example.org/onto/">
  <owl:Class rdf:about="http://example.org/onto/class/google_apigee_environment">
    <rdfs:label>google_apigee_environment</rdfs:label>
    <rdfs:comment>#
#     ***     AUTO GENERATED CODE    ***    Type: MMv1     ***
#
# ----------------------------------------------------------------------------
#
#     This code is generated by Magic Modules using the following:
#
#     Configuration: https:#github.com/GoogleCloudPlatform/magic-modules/tree/main/mmv1/products/apigee/Environment.yaml
#     Template:      https:#github.com/GoogleCloudPlatform/magic-modules/tree/main/mmv1/templates/terraform/resource.html.markdown.tmpl
#
#     DO NOT EDIT this file directly. Any changes made to this file will be
#     overwritten during the next generation cycle.
#
# ----------------------------------------------------------------------------
subcategory: "Apigee"
description: |-
  An `Environment` in Apigee.
---</rdfs:comment>
  </owl:Class>
  <owl:DatatypeProperty rdf:about="http://example.org/onto/prop/google_apigee_environment_api_proxy_type">
    <rdfs:label>api_proxy_type</rdfs:label>
    <rdfs:comment>Optional. API Proxy type supported by the environment. The type can be set when creating
the Environment and cannot be changed. Possible values: ["API_PROXY_TYPE_UNSPECIFIED", "PROGRAMMABLE", "CONFIGURABLE"]</rdfs:comment>
    <rdfs:domain rdf:resource="http://example.org/onto/class/google_apigee_environment"/>
    <rdfs:range rdf:resource="http://www.w3.org/2001/XMLSchema#string"/>
  </owl:DatatypeProperty>
  <owl:DatatypeProperty rdf:about="http://example.org/onto/prop/google_apigee_environment_deployment_type">
    <rdfs:label>deployment_type</rdfs:label>
    <rdfs:comment>Optional. Deployment type supported by the environment. The deployment type can be
set when creating the environment and cannot be changed. When you enable archive
deployment, you will be prevented from performing a subset of actions within the
environment, including:
Managing the deployment of API proxy or shared flow revisions;
Creating, updating, or deleting resource files;
Creating, updating, or deleting target servers. Possible values: ["DEPLOYMENT_TYPE_UNSPECIFIED", "PROXY", "ARCHIVE"]</rdfs:comment>
    <rdfs:domain rdf:resource="http://example.org/onto/class/google_apigee_environment"/>
    <rdfs:range rdf:resource="http://www.w3.org/2001/XMLSchema#string"/>
  </owl:DatatypeProperty>
  <owl:DatatypeProperty rdf:about="http://example.org/onto/prop/google_apigee_environment_description">
    <rdfs:label>description</rdfs:label>
    <rdfs:comment>Description of the environment.</rdfs:comment>
    <rdfs:domain rdf:resource="http://example.org/onto/class/google_apigee_environment"/>
    <rdfs:range rdf:resource="http://www.w3.org/2001/XMLSchema#string"/>
  </owl:DatatypeProperty>
  <owl:DatatypeProperty rdf:about="http://example.org/onto/prop/google_apigee_environment_display_name">
    <rdfs:label>display_name</rdfs:label>
    <rdfs:comment>Display name of the environment.</rdfs:comment>
    <rdfs:domain rdf:resource="http://example.org/onto/class/google_apigee_environment"/>
    <rdfs:range rdf:resource="http://www.w3.org/2001/XMLSchema#string"/>
  </owl:DatatypeProperty>
  <owl:DatatypeProperty rdf:about="http://example.org/onto/prop/google_apigee_environment_forward_proxy_uri">
    <rdfs:label>forward_proxy_uri</rdfs:label>
    <rdfs:comment>Optional. URI of the forward proxy to be applied to the runtime instances in this environment. Must be in the format of {scheme}://{hostname}:{port}. Note that the scheme must be one of "http" or "https", and the port must be supplied.</rdfs:comment>
    <rdfs:domain rdf:resource="http://example.org/onto/class/google_apigee_environment"/>
    <rdfs:range rdf:resource="http://www.w3.org/2001/XMLSchema#string"/>
  </owl:DatatypeProperty>
  <owl:DatatypeProperty rdf:about="http://example.org/onto/prop/google_apigee_environment_id">
    <rdfs:label>id</rdfs:label>
    <rdfs:domain rdf:resource="http://example.org/onto/class/google_apigee_environment"/>
    <rdfs:range rdf:resource="http://www.w3.org/2001/XMLSchema#string"/>
  </owl:DatatypeProperty>
  <owl:DatatypeProperty rdf:about="http://example.org/onto/prop/google_apigee_environment_name">
    <rdfs:label>name</rdfs:label>
    <rdfs:comment>The resource ID of the environment.</rdfs:comment>
    <rdfs:domain rdf:resource="http://example.org/onto/class/google_apigee_environment"/>
    <rdfs:range rdf:resource="http://www.w3.org/2001/XMLSchema#string"/>
  </owl:DatatypeProperty>
  <owl:DatatypeProperty rdf:about="http://example.org/onto/prop/google_apigee_environment_org_id">
    <rdfs:label>org_id</rdfs:label>
    <rdfs:comment>The Apigee Organization associated with the Apigee environment,
in the format 'organizations/{{org_name}}'.</rdfs:comment>
    <rdfs:domain rdf:resource="http://example.org/onto/class/google_apigee_environment"/>
    <rdfs:range rdf:resource="http://www.w3.org/2001/XMLSchema#string"/>
  </owl:DatatypeProperty>
  <owl:DatatypeProperty rdf:about="http://example.org/onto/prop/google_apigee_environment_type">
    <rdfs:label>type</rdfs:label>
    <rdfs:comment>Types that can be selected for an Environment. Each of the types are
limited by capability and capacity. Refer to Apigee's public documentation
to understand about each of these types in details.
An Apigee org can support heterogeneous Environments. Possible values: ["ENVIRONMENT_TYPE_UNSPECIFIED", "BASE", "INTERMEDIATE", "COMPREHENSIVE"]</rdfs:comment>
    <rdfs:domain rdf:resource="http://example.org/onto/class/google_apigee_environment"/>
    <rdfs:range rdf:resource="http://www.w3.org/2001/XMLSchema#string"/>
  </owl:DatatypeProperty>
  <owl:DatatypeProperty rdf:about="http://example.org/onto/prop/google_apigee_environment_ip_header_index">
    <rdfs:label>ip_header_index</rdfs:label>
    <rdfs:comment>The index of the ip in the header. Positive indices 0, 1, 2, 3 chooses indices from the left (first ips). Negative indices -1, -2, -3 chooses indices from the right (last ips).</rdfs:comment>
    <rdfs:domain rdf:resource="http://example.org/onto/class/google_apigee_environment"/>
    <rdfs:range rdf:resource="http://www.w3.org/2001/XMLSchema#string"/>
  </owl:DatatypeProperty>
  <owl:DatatypeProperty rdf:about="http://example.org/onto/prop/google_apigee_environment_ip_header_name">
    <rdfs:label>ip_header_name</rdfs:label>
    <rdfs:comment>The name of the header to extract the client ip from. We are currently only supporting the X-Forwarded-For header.</rdfs:comment>
    <rdfs:domain rdf:resource="http://example.org/onto/class/google_apigee_environment"/>
    <rdfs:range rdf:resource="http://www.w3.org/2001/XMLSchema#string"/>
  </owl:DatatypeProperty>
  <owl:DatatypeProperty rdf:about="http://example.org/onto/prop/google_apigee_environment_current_aggregate_node_count">
    <rdfs:label>current_aggregate_node_count</rdfs:label>
    <rdfs:comment>The current total number of gateway nodes that each environment currently has across
all instances.</rdfs:comment>
    <rdfs:domain rdf:resource="http://example.org/onto/class/google_apigee_environment"/>
    <rdfs:range rdf:resource="http://www.w3.org/2001/XMLSchema#string"/>
  </owl:DatatypeProperty>
  <owl:DatatypeProperty rdf:about="http://example.org/onto/prop/google_apigee_environment_max_node_count">
    <rdfs:label>max_node_count</rdfs:label>
    <rdfs:comment>The maximum total number of gateway nodes that the is reserved for all instances that
has the specified environment. If not specified, the default is determined by the
recommended maximum number of nodes for that gateway.</rdfs:comment>
    <rdfs:domain rdf:resource="http://example.org/onto/class/google_apigee_environment"/>
    <rdfs:range rdf:resource="http://www.w3.org/2001/XMLSchema#string"/>
  </owl:DatatypeProperty>
  <owl:DatatypeProperty rdf:about="http://example.org/onto/prop/google_apigee_environment_min_node_count">
    <rdfs:label>min_node_count</rdfs:label>
    <rdfs:comment>The minimum total number of gateway nodes that the is reserved for all instances that
has the specified environment. If not specified, the default is determined by the
recommended minimum number of nodes for that gateway.</rdfs:comment>
    <rdfs:domain rdf:resource="http://example.org/onto/class/google_apigee_environment"/>
    <rdfs:range rdf:resource="http://www.w3.org/2001/XMLSchema#string"/>
  </owl:DatatypeProperty>
  <owl:DatatypeProperty rdf:about="http://example.org/onto/prop/google_apigee_environment_name">
    <rdfs:label>name</rdfs:label>
    <rdfs:comment>The property key.</rdfs:comment>
    <rdfs:domain rdf:resource="http://example.org/onto/class/google_apigee_environment"/>
    <rdfs:range rdf:resource="http://www.w3.org/2001/XMLSchema#string"/>
  </owl:DatatypeProperty>
  <owl:DatatypeProperty rdf:about="http://example.org/onto/prop/google_apigee_environment_value">
    <rdfs:label>value</rdfs:label>
    <rdfs:comment>The property value.</rdfs:comment>
    <rdfs:domain rdf:resource="http://example.org/onto/class/google_apigee_environment"/>
    <rdfs:range rdf:resource="http://www.w3.org/2001/XMLSchema#string"/>
  </owl:DatatypeProperty>
  <owl:DatatypeProperty rdf:about="http://example.org/onto/prop/google_apigee_environment_create">
    <rdfs:label>create</rdfs:label>
    <rdfs:domain rdf:resource="http://example.org/onto/class/google_apigee_environment"/>
    <rdfs:range rdf:resource="http://www.w3.org/2001/XMLSchema#string"/>
  </owl:DatatypeProperty>
  <owl:DatatypeProperty rdf:about="http://example.org/onto/prop/google_apigee_environment_delete">
    <rdfs:label>delete</rdfs:label>
    <rdfs:domain rdf:resource="http://example.org/onto/class/google_apigee_environment"/>
    <rdfs:range rdf:resource="http://www.w3.org/2001/XMLSchema#string"/>
  </owl:DatatypeProperty>
  <owl:DatatypeProperty rdf:about="http://example.org/onto/prop/google_apigee_environment_update">
    <rdfs:label>update</rdfs:label>
    <rdfs:domain rdf:resource="http://example.org/onto/class/google_apigee_environment"/>
    <rdfs:range rdf:resource="http://www.w3.org/2001/XMLSchema#string"/>
  </owl:DatatypeProperty>
</rdf:RDF>
