<?xml version="1.0" encoding="UTF-8"?>
<rdf:RDF
  xmlns:rdf="http://www.w3.org/1999/02/22-rdf-syntax-ns#"
  xmlns:rdfs="http://www.w3.org/2000/01/rdf-schema#"
  xmlns:owl="http://www.w3.org/2002/07/owl#"
  xmlns:xsd="http://www.w3.org/2001/XMLSchema#"
  xml:base="http://example.org/onto/">
  <owl:Class rdf:about="http://example.org/onto/class/google_access_context_manager_access_level">
    <rdfs:label>google_access_context_manager_access_level</rdfs:label>
    <rdfs:comment>#
#     ***     AUTO GENERATED CODE    ***    Type: MMv1     ***
#
# ----------------------------------------------------------------------------
#
#     This code is generated by Magic Modules using the following:
#
#     Configuration: https:#github.com/GoogleCloudPlatform/magic-modules/tree/main/mmv1/products/accesscontextmanager/AccessLevel.yaml
#     Template:      https:#github.com/GoogleCloudPlatform/magic-modules/tree/main/mmv1/templates/terraform/resource.html.markdown.tmpl
#
#     DO NOT EDIT this file directly. Any changes made to this file will be
#     overwritten during the next generation cycle.
#
# ----------------------------------------------------------------------------
subcategory: "Access Context Manager (VPC Service Controls)"
description: |-
  An AccessLevel is a label that can be applied to requests to GCP services,
  along with a list of requirements necessary for the label to be applied.
---</rdfs:comment>
  </owl:Class>
  <owl:DatatypeProperty rdf:about="http://example.org/onto/prop/google_access_context_manager_access_level_description">
    <rdfs:label>description</rdfs:label>
    <rdfs:comment>Description of the AccessLevel and its use. Does not affect behavior.</rdfs:comment>
    <rdfs:domain rdf:resource="http://example.org/onto/class/google_access_context_manager_access_level"/>
    <rdfs:range rdf:resource="http://www.w3.org/2001/XMLSchema#string"/>
  </owl:DatatypeProperty>
  <owl:DatatypeProperty rdf:about="http://example.org/onto/prop/google_access_context_manager_access_level_id">
    <rdfs:label>id</rdfs:label>
    <rdfs:domain rdf:resource="http://example.org/onto/class/google_access_context_manager_access_level"/>
    <rdfs:range rdf:resource="http://www.w3.org/2001/XMLSchema#string"/>
  </owl:DatatypeProperty>
  <owl:DatatypeProperty rdf:about="http://example.org/onto/prop/google_access_context_manager_access_level_name">
    <rdfs:label>name</rdfs:label>
    <rdfs:comment>Resource name for the Access Level. The short_name component must begin
with a letter and only include alphanumeric and '_'.
Format: accessPolicies/{policy_id}/accessLevels/{short_name}</rdfs:comment>
    <rdfs:domain rdf:resource="http://example.org/onto/class/google_access_context_manager_access_level"/>
    <rdfs:range rdf:resource="http://www.w3.org/2001/XMLSchema#string"/>
  </owl:DatatypeProperty>
  <owl:DatatypeProperty rdf:about="http://example.org/onto/prop/google_access_context_manager_access_level_parent">
    <rdfs:label>parent</rdfs:label>
    <rdfs:comment>The AccessPolicy this AccessLevel lives in.
Format: accessPolicies/{policy_id}</rdfs:comment>
    <rdfs:domain rdf:resource="http://example.org/onto/class/google_access_context_manager_access_level"/>
    <rdfs:range rdf:resource="http://www.w3.org/2001/XMLSchema#string"/>
  </owl:DatatypeProperty>
  <owl:DatatypeProperty rdf:about="http://example.org/onto/prop/google_access_context_manager_access_level_title">
    <rdfs:label>title</rdfs:label>
    <rdfs:comment>Human readable title. Must be unique within the Policy.</rdfs:comment>
    <rdfs:domain rdf:resource="http://example.org/onto/class/google_access_context_manager_access_level"/>
    <rdfs:range rdf:resource="http://www.w3.org/2001/XMLSchema#string"/>
  </owl:DatatypeProperty>
  <owl:DatatypeProperty rdf:about="http://example.org/onto/prop/google_access_context_manager_access_level_combining_function">
    <rdfs:label>combining_function</rdfs:label>
    <rdfs:comment>How the conditions list should be combined to determine if a request
is granted this AccessLevel. If AND is used, each Condition in
conditions must be satisfied for the AccessLevel to be applied. If
OR is used, at least one Condition in conditions must be satisfied
for the AccessLevel to be applied. Default value: "AND" Possible values: ["AND", "OR"]</rdfs:comment>
    <rdfs:domain rdf:resource="http://example.org/onto/class/google_access_context_manager_access_level"/>
    <rdfs:range rdf:resource="http://www.w3.org/2001/XMLSchema#string"/>
  </owl:DatatypeProperty>
  <owl:DatatypeProperty rdf:about="http://example.org/onto/prop/google_access_context_manager_access_level_ip_subnetworks">
    <rdfs:label>ip_subnetworks</rdfs:label>
    <rdfs:comment>A list of CIDR block IP subnetwork specification. May be IPv4
or IPv6.
Note that for a CIDR IP address block, the specified IP address
portion must be properly truncated (i.e. all the host bits must
be zero) or the input is considered malformed. For example,
"192.0.2.0/24" is accepted but "192.0.2.1/24" is not. Similarly,
for IPv6, "2001:db8::/32" is accepted whereas "2001:db8::1/32"
is not. The originating IP of a request must be in one of the
listed subnets in order for this Condition to be true.
If empty, all IP addresses are allowed.</rdfs:comment>
    <rdfs:domain rdf:resource="http://example.org/onto/class/google_access_context_manager_access_level"/>
    <rdfs:range rdf:resource="http://www.w3.org/2001/XMLSchema#string"/>
  </owl:DatatypeProperty>
  <owl:DatatypeProperty rdf:about="http://example.org/onto/prop/google_access_context_manager_access_level_members">
    <rdfs:label>members</rdfs:label>
    <rdfs:comment>An allowed list of members (users, service accounts).
Using groups is not supported yet.

The signed-in user originating the request must be a part of one
of the provided members. If not specified, a request may come
from any user (logged in/not logged in, not present in any
groups, etc.).
Formats: 'user:{emailid}', 'serviceAccount:{emailid}'</rdfs:comment>
    <rdfs:domain rdf:resource="http://example.org/onto/class/google_access_context_manager_access_level"/>
    <rdfs:range rdf:resource="http://www.w3.org/2001/XMLSchema#string"/>
  </owl:DatatypeProperty>
  <owl:DatatypeProperty rdf:about="http://example.org/onto/prop/google_access_context_manager_access_level_negate">
    <rdfs:label>negate</rdfs:label>
    <rdfs:comment>Whether to negate the Condition. If true, the Condition becomes
a NAND over its non-empty fields, each field must be false for
the Condition overall to be satisfied. Defaults to false.</rdfs:comment>
    <rdfs:domain rdf:resource="http://example.org/onto/class/google_access_context_manager_access_level"/>
    <rdfs:range rdf:resource="http://www.w3.org/2001/XMLSchema#string"/>
  </owl:DatatypeProperty>
  <owl:DatatypeProperty rdf:about="http://example.org/onto/prop/google_access_context_manager_access_level_regions">
    <rdfs:label>regions</rdfs:label>
    <rdfs:comment>The request must originate from one of the provided
countries/regions.
Format: A valid ISO 3166-1 alpha-2 code.</rdfs:comment>
    <rdfs:domain rdf:resource="http://example.org/onto/class/google_access_context_manager_access_level"/>
    <rdfs:range rdf:resource="http://www.w3.org/2001/XMLSchema#string"/>
  </owl:DatatypeProperty>
  <owl:DatatypeProperty rdf:about="http://example.org/onto/prop/google_access_context_manager_access_level_required_access_levels">
    <rdfs:label>required_access_levels</rdfs:label>
    <rdfs:comment>A list of other access levels defined in the same Policy,
referenced by resource name. Referencing an AccessLevel which
does not exist is an error. All access levels listed must be
granted for the Condition to be true.
Format: accessPolicies/{policy_id}/accessLevels/{short_name}</rdfs:comment>
    <rdfs:domain rdf:resource="http://example.org/onto/class/google_access_context_manager_access_level"/>
    <rdfs:range rdf:resource="http://www.w3.org/2001/XMLSchema#string"/>
  </owl:DatatypeProperty>
  <owl:DatatypeProperty rdf:about="http://example.org/onto/prop/google_access_context_manager_access_level_allowed_device_management_levels">
    <rdfs:label>allowed_device_management_levels</rdfs:label>
    <rdfs:comment>A list of allowed device management levels.
An empty list allows all management levels. Possible values: ["MANAGEMENT_UNSPECIFIED", "NONE", "BASIC", "COMPLETE"]</rdfs:comment>
    <rdfs:domain rdf:resource="http://example.org/onto/class/google_access_context_manager_access_level"/>
    <rdfs:range rdf:resource="http://www.w3.org/2001/XMLSchema#string"/>
  </owl:DatatypeProperty>
  <owl:DatatypeProperty rdf:about="http://example.org/onto/prop/google_access_context_manager_access_level_allowed_encryption_statuses">
    <rdfs:label>allowed_encryption_statuses</rdfs:label>
    <rdfs:comment>A list of allowed encryptions statuses.
An empty list allows all statuses. Possible values: ["ENCRYPTION_UNSPECIFIED", "ENCRYPTION_UNSUPPORTED", "UNENCRYPTED", "ENCRYPTED"]</rdfs:comment>
    <rdfs:domain rdf:resource="http://example.org/onto/class/google_access_context_manager_access_level"/>
    <rdfs:range rdf:resource="http://www.w3.org/2001/XMLSchema#string"/>
  </owl:DatatypeProperty>
  <owl:DatatypeProperty rdf:about="http://example.org/onto/prop/google_access_context_manager_access_level_require_admin_approval">
    <rdfs:label>require_admin_approval</rdfs:label>
    <rdfs:comment>Whether the device needs to be approved by the customer admin.</rdfs:comment>
    <rdfs:domain rdf:resource="http://example.org/onto/class/google_access_context_manager_access_level"/>
    <rdfs:range rdf:resource="http://www.w3.org/2001/XMLSchema#string"/>
  </owl:DatatypeProperty>
  <owl:DatatypeProperty rdf:about="http://example.org/onto/prop/google_access_context_manager_access_level_require_corp_owned">
    <rdfs:label>require_corp_owned</rdfs:label>
    <rdfs:comment>Whether the device needs to be corp owned.</rdfs:comment>
    <rdfs:domain rdf:resource="http://example.org/onto/class/google_access_context_manager_access_level"/>
    <rdfs:range rdf:resource="http://www.w3.org/2001/XMLSchema#string"/>
  </owl:DatatypeProperty>
  <owl:DatatypeProperty rdf:about="http://example.org/onto/prop/google_access_context_manager_access_level_require_screen_lock">
    <rdfs:label>require_screen_lock</rdfs:label>
    <rdfs:comment>Whether or not screenlock is required for the DevicePolicy
to be true. Defaults to false.</rdfs:comment>
    <rdfs:domain rdf:resource="http://example.org/onto/class/google_access_context_manager_access_level"/>
    <rdfs:range rdf:resource="http://www.w3.org/2001/XMLSchema#string"/>
  </owl:DatatypeProperty>
  <owl:DatatypeProperty rdf:about="http://example.org/onto/prop/google_access_context_manager_access_level_minimum_version">
    <rdfs:label>minimum_version</rdfs:label>
    <rdfs:comment>The minimum allowed OS version. If not set, any version
of this OS satisfies the constraint.
Format: "major.minor.patch" such as "10.5.301", "9.2.1".</rdfs:comment>
    <rdfs:domain rdf:resource="http://example.org/onto/class/google_access_context_manager_access_level"/>
    <rdfs:range rdf:resource="http://www.w3.org/2001/XMLSchema#string"/>
  </owl:DatatypeProperty>
  <owl:DatatypeProperty rdf:about="http://example.org/onto/prop/google_access_context_manager_access_level_os_type">
    <rdfs:label>os_type</rdfs:label>
    <rdfs:comment>The operating system type of the device. Possible values: ["OS_UNSPECIFIED", "DESKTOP_MAC", "DESKTOP_WINDOWS", "DESKTOP_LINUX", "DESKTOP_CHROME_OS", "ANDROID", "IOS"]</rdfs:comment>
    <rdfs:domain rdf:resource="http://example.org/onto/class/google_access_context_manager_access_level"/>
    <rdfs:range rdf:resource="http://www.w3.org/2001/XMLSchema#string"/>
  </owl:DatatypeProperty>
  <owl:DatatypeProperty rdf:about="http://example.org/onto/prop/google_access_context_manager_access_level_require_verified_chrome_os">
    <rdfs:label>require_verified_chrome_os</rdfs:label>
    <rdfs:comment>If you specify DESKTOP_CHROME_OS for osType, you can optionally include requireVerifiedChromeOs to require Chrome Verified Access.</rdfs:comment>
    <rdfs:domain rdf:resource="http://example.org/onto/class/google_access_context_manager_access_level"/>
    <rdfs:range rdf:resource="http://www.w3.org/2001/XMLSchema#string"/>
  </owl:DatatypeProperty>
  <owl:DatatypeProperty rdf:about="http://example.org/onto/prop/google_access_context_manager_access_level_network">
    <rdfs:label>network</rdfs:label>
    <rdfs:comment>Required. Network name to be allowed by this Access Level. Networks of foreign organizations requires 'compute.network.get' permission to be granted to caller.</rdfs:comment>
    <rdfs:domain rdf:resource="http://example.org/onto/class/google_access_context_manager_access_level"/>
    <rdfs:range rdf:resource="http://www.w3.org/2001/XMLSchema#string"/>
  </owl:DatatypeProperty>
  <owl:DatatypeProperty rdf:about="http://example.org/onto/prop/google_access_context_manager_access_level_vpc_ip_subnetworks">
    <rdfs:label>vpc_ip_subnetworks</rdfs:label>
    <rdfs:comment>A list of CIDR block IP subnetwork specification. Must be IPv4.</rdfs:comment>
    <rdfs:domain rdf:resource="http://example.org/onto/class/google_access_context_manager_access_level"/>
    <rdfs:range rdf:resource="http://www.w3.org/2001/XMLSchema#string"/>
  </owl:DatatypeProperty>
  <owl:DatatypeProperty rdf:about="http://example.org/onto/prop/google_access_context_manager_access_level_description">
    <rdfs:label>description</rdfs:label>
    <rdfs:comment>Description of the expression</rdfs:comment>
    <rdfs:domain rdf:resource="http://example.org/onto/class/google_access_context_manager_access_level"/>
    <rdfs:range rdf:resource="http://www.w3.org/2001/XMLSchema#string"/>
  </owl:DatatypeProperty>
  <owl:DatatypeProperty rdf:about="http://example.org/onto/prop/google_access_context_manager_access_level_expression">
    <rdfs:label>expression</rdfs:label>
    <rdfs:comment>Textual representation of an expression in Common Expression Language syntax.</rdfs:comment>
    <rdfs:domain rdf:resource="http://example.org/onto/class/google_access_context_manager_access_level"/>
    <rdfs:range rdf:resource="http://www.w3.org/2001/XMLSchema#string"/>
  </owl:DatatypeProperty>
  <owl:DatatypeProperty rdf:about="http://example.org/onto/prop/google_access_context_manager_access_level_location">
    <rdfs:label>location</rdfs:label>
    <rdfs:comment>String indicating the location of the expression for error reporting, e.g. a file name and a position in the file</rdfs:comment>
    <rdfs:domain rdf:resource="http://example.org/onto/class/google_access_context_manager_access_level"/>
    <rdfs:range rdf:resource="http://www.w3.org/2001/XMLSchema#string"/>
  </owl:DatatypeProperty>
  <owl:DatatypeProperty rdf:about="http://example.org/onto/prop/google_access_context_manager_access_level_title">
    <rdfs:label>title</rdfs:label>
    <rdfs:comment>Title for the expression, i.e. a short string describing its purpose.</rdfs:comment>
    <rdfs:domain rdf:resource="http://example.org/onto/class/google_access_context_manager_access_level"/>
    <rdfs:range rdf:resource="http://www.w3.org/2001/XMLSchema#string"/>
  </owl:DatatypeProperty>
  <owl:DatatypeProperty rdf:about="http://example.org/onto/prop/google_access_context_manager_access_level_create">
    <rdfs:label>create</rdfs:label>
    <rdfs:domain rdf:resource="http://example.org/onto/class/google_access_context_manager_access_level"/>
    <rdfs:range rdf:resource="http://www.w3.org/2001/XMLSchema#string"/>
  </owl:DatatypeProperty>
  <owl:DatatypeProperty rdf:about="http://example.org/onto/prop/google_access_context_manager_access_level_delete">
    <rdfs:label>delete</rdfs:label>
    <rdfs:domain rdf:resource="http://example.org/onto/class/google_access_context_manager_access_level"/>
    <rdfs:range rdf:resource="http://www.w3.org/2001/XMLSchema#string"/>
  </owl:DatatypeProperty>
  <owl:DatatypeProperty rdf:about="http://example.org/onto/prop/google_access_context_manager_access_level_update">
    <rdfs:label>update</rdfs:label>
    <rdfs:domain rdf:resource="http://example.org/onto/class/google_access_context_manager_access_level"/>
    <rdfs:range rdf:resource="http://www.w3.org/2001/XMLSchema#string"/>
  </owl:DatatypeProperty>
</rdf:RDF>
