<?xml version="1.0" encoding="UTF-8"?>
<rdf:RDF
  xmlns:rdf="http://www.w3.org/1999/02/22-rdf-syntax-ns#"
  xmlns:rdfs="http://www.w3.org/2000/01/rdf-schema#"
  xmlns:owl="http://www.w3.org/2002/07/owl#"
  xmlns:xsd="http://www.w3.org/2001/XMLSchema#"
  xml:base="http://example.org/onto/">
  <owl:Class rdf:about="http://example.org/onto/class/google_data_catalog_entry">
    <rdfs:label>google_data_catalog_entry</rdfs:label>
    <rdfs:comment>#
#     ***     AUTO GENERATED CODE    ***    Type: MMv1     ***
#
# ----------------------------------------------------------------------------
#
#     This code is generated by Magic Modules using the following:
#
#     Configuration: https:#github.com/GoogleCloudPlatform/magic-modules/tree/main/mmv1/products/datacatalog/Entry.yaml
#     Template:      https:#github.com/GoogleCloudPlatform/magic-modules/tree/main/mmv1/templates/terraform/resource.html.markdown.tmpl
#
#     DO NOT EDIT this file directly. Any changes made to this file will be
#     overwritten during the next generation cycle.
#
# ----------------------------------------------------------------------------
subcategory: "Data Catalog"
description: |-
  Entry Metadata.
---</rdfs:comment>
  </owl:Class>
  <owl:DatatypeProperty rdf:about="http://example.org/onto/prop/google_data_catalog_entry_bigquery_date_sharded_spec">
    <rdfs:label>bigquery_date_sharded_spec</rdfs:label>
    <rdfs:comment>Specification for a group of BigQuery tables with name pattern [prefix]YYYYMMDD.
Context: https://cloud.google.com/bigquery/docs/partitioned-tables#partitioning_versus_sharding.</rdfs:comment>
    <rdfs:domain rdf:resource="http://example.org/onto/class/google_data_catalog_entry"/>
    <rdfs:range rdf:resource="http://www.w3.org/2001/XMLSchema#string"/>
  </owl:DatatypeProperty>
  <owl:DatatypeProperty rdf:about="http://example.org/onto/prop/google_data_catalog_entry_bigquery_table_spec">
    <rdfs:label>bigquery_table_spec</rdfs:label>
    <rdfs:comment>Specification that applies to a BigQuery table. This is only valid on entries of type TABLE.</rdfs:comment>
    <rdfs:domain rdf:resource="http://example.org/onto/class/google_data_catalog_entry"/>
    <rdfs:range rdf:resource="http://www.w3.org/2001/XMLSchema#string"/>
  </owl:DatatypeProperty>
  <owl:DatatypeProperty rdf:about="http://example.org/onto/prop/google_data_catalog_entry_description">
    <rdfs:label>description</rdfs:label>
    <rdfs:comment>Entry description, which can consist of several sentences or paragraphs that describe entry contents.</rdfs:comment>
    <rdfs:domain rdf:resource="http://example.org/onto/class/google_data_catalog_entry"/>
    <rdfs:range rdf:resource="http://www.w3.org/2001/XMLSchema#string"/>
  </owl:DatatypeProperty>
  <owl:DatatypeProperty rdf:about="http://example.org/onto/prop/google_data_catalog_entry_display_name">
    <rdfs:label>display_name</rdfs:label>
    <rdfs:comment>Display information such as title and description. A short name to identify the entry,
for example, "Analytics Data - Jan 2011".</rdfs:comment>
    <rdfs:domain rdf:resource="http://example.org/onto/class/google_data_catalog_entry"/>
    <rdfs:range rdf:resource="http://www.w3.org/2001/XMLSchema#string"/>
  </owl:DatatypeProperty>
  <owl:DatatypeProperty rdf:about="http://example.org/onto/prop/google_data_catalog_entry_entry_group">
    <rdfs:label>entry_group</rdfs:label>
    <rdfs:comment>The name of the entry group this entry is in.</rdfs:comment>
    <rdfs:domain rdf:resource="http://example.org/onto/class/google_data_catalog_entry"/>
    <rdfs:range rdf:resource="http://www.w3.org/2001/XMLSchema#string"/>
  </owl:DatatypeProperty>
  <owl:DatatypeProperty rdf:about="http://example.org/onto/prop/google_data_catalog_entry_entry_id">
    <rdfs:label>entry_id</rdfs:label>
    <rdfs:comment>The id of the entry to create.</rdfs:comment>
    <rdfs:domain rdf:resource="http://example.org/onto/class/google_data_catalog_entry"/>
    <rdfs:range rdf:resource="http://www.w3.org/2001/XMLSchema#string"/>
  </owl:DatatypeProperty>
  <owl:DatatypeProperty rdf:about="http://example.org/onto/prop/google_data_catalog_entry_id">
    <rdfs:label>id</rdfs:label>
    <rdfs:domain rdf:resource="http://example.org/onto/class/google_data_catalog_entry"/>
    <rdfs:range rdf:resource="http://www.w3.org/2001/XMLSchema#string"/>
  </owl:DatatypeProperty>
  <owl:DatatypeProperty rdf:about="http://example.org/onto/prop/google_data_catalog_entry_integrated_system">
    <rdfs:label>integrated_system</rdfs:label>
    <rdfs:comment>This field indicates the entry's source system that Data Catalog integrates with, such as BigQuery or Pub/Sub.</rdfs:comment>
    <rdfs:domain rdf:resource="http://example.org/onto/class/google_data_catalog_entry"/>
    <rdfs:range rdf:resource="http://www.w3.org/2001/XMLSchema#string"/>
  </owl:DatatypeProperty>
  <owl:DatatypeProperty rdf:about="http://example.org/onto/prop/google_data_catalog_entry_linked_resource">
    <rdfs:label>linked_resource</rdfs:label>
    <rdfs:comment>The resource this metadata entry refers to.
For Google Cloud Platform resources, linkedResource is the full name of the resource.
For example, the linkedResource for a table resource from BigQuery is:
//bigquery.googleapis.com/projects/projectId/datasets/datasetId/tables/tableId
Output only when Entry is of type in the EntryType enum. For entries with userSpecifiedType,
this field is optional and defaults to an empty string.</rdfs:comment>
    <rdfs:domain rdf:resource="http://example.org/onto/class/google_data_catalog_entry"/>
    <rdfs:range rdf:resource="http://www.w3.org/2001/XMLSchema#string"/>
  </owl:DatatypeProperty>
  <owl:DatatypeProperty rdf:about="http://example.org/onto/prop/google_data_catalog_entry_name">
    <rdfs:label>name</rdfs:label>
    <rdfs:comment>The Data Catalog resource name of the entry in URL format.
Example: projects/{project_id}/locations/{location}/entryGroups/{entryGroupId}/entries/{entryId}.
Note that this Entry and its child resources may not actually be stored in the location in this name.</rdfs:comment>
    <rdfs:domain rdf:resource="http://example.org/onto/class/google_data_catalog_entry"/>
    <rdfs:range rdf:resource="http://www.w3.org/2001/XMLSchema#string"/>
  </owl:DatatypeProperty>
  <owl:DatatypeProperty rdf:about="http://example.org/onto/prop/google_data_catalog_entry_schema">
    <rdfs:label>schema</rdfs:label>
    <rdfs:comment>Schema of the entry (e.g. BigQuery, GoogleSQL, Avro schema), as a json string. An entry might not have any schema
attached to it. See
https://cloud.google.com/data-catalog/docs/reference/rest/v1/projects.locations.entryGroups.entries#schema
for what fields this schema can contain.</rdfs:comment>
    <rdfs:domain rdf:resource="http://example.org/onto/class/google_data_catalog_entry"/>
    <rdfs:range rdf:resource="http://www.w3.org/2001/XMLSchema#string"/>
  </owl:DatatypeProperty>
  <owl:DatatypeProperty rdf:about="http://example.org/onto/prop/google_data_catalog_entry_type">
    <rdfs:label>type</rdfs:label>
    <rdfs:comment>The type of the entry. Only used for Entries with types in the EntryType enum.
Currently, only FILESET enum value is allowed. All other entries created through Data Catalog must use userSpecifiedType. Possible values: ["FILESET"]</rdfs:comment>
    <rdfs:domain rdf:resource="http://example.org/onto/class/google_data_catalog_entry"/>
    <rdfs:range rdf:resource="http://www.w3.org/2001/XMLSchema#string"/>
  </owl:DatatypeProperty>
  <owl:DatatypeProperty rdf:about="http://example.org/onto/prop/google_data_catalog_entry_user_specified_system">
    <rdfs:label>user_specified_system</rdfs:label>
    <rdfs:comment>This field indicates the entry's source system that Data Catalog does not integrate with.
userSpecifiedSystem strings must begin with a letter or underscore and can only contain letters, numbers,
and underscores; are case insensitive; must be at least 1 character and at most 64 characters long.</rdfs:comment>
    <rdfs:domain rdf:resource="http://example.org/onto/class/google_data_catalog_entry"/>
    <rdfs:range rdf:resource="http://www.w3.org/2001/XMLSchema#string"/>
  </owl:DatatypeProperty>
  <owl:DatatypeProperty rdf:about="http://example.org/onto/prop/google_data_catalog_entry_user_specified_type">
    <rdfs:label>user_specified_type</rdfs:label>
    <rdfs:comment>Entry type if it does not fit any of the input-allowed values listed in EntryType enum above.
When creating an entry, users should check the enum values first, if nothing matches the entry
to be created, then provide a custom value, for example "my_special_type".
userSpecifiedType strings must begin with a letter or underscore and can only contain letters,
numbers, and underscores; are case insensitive; must be at least 1 character and at most 64 characters long.</rdfs:comment>
    <rdfs:domain rdf:resource="http://example.org/onto/class/google_data_catalog_entry"/>
    <rdfs:range rdf:resource="http://www.w3.org/2001/XMLSchema#string"/>
  </owl:DatatypeProperty>
  <owl:DatatypeProperty rdf:about="http://example.org/onto/prop/google_data_catalog_entry_file_patterns">
    <rdfs:label>file_patterns</rdfs:label>
    <rdfs:comment>Patterns to identify a set of files in Google Cloud Storage.
See [Cloud Storage documentation](https://cloud.google.com/storage/docs/gsutil/addlhelp/WildcardNames)
for more information. Note that bucket wildcards are currently not supported. Examples of valid filePatterns:

* gs://bucket_name/dir/*: matches all files within bucket_name/dir directory.
* gs://bucket_name/dir/**: matches all files in bucket_name/dir spanning all subdirectories.
* gs://bucket_name/file*: matches files prefixed by file in bucket_name
* gs://bucket_name/??.txt: matches files with two characters followed by .txt in bucket_name
* gs://bucket_name/[aeiou].txt: matches files that contain a single vowel character followed by .txt in bucket_name
* gs://bucket_name/[a-m].txt: matches files that contain a, b, ... or m followed by .txt in bucket_name
* gs://bucket_name/a/*/b: matches all files in bucket_name that match a/*/b pattern, such as a/c/b, a/d/b
* gs://another_bucket/a.txt: matches gs://another_bucket/a.txt</rdfs:comment>
    <rdfs:domain rdf:resource="http://example.org/onto/class/google_data_catalog_entry"/>
    <rdfs:range rdf:resource="http://www.w3.org/2001/XMLSchema#string"/>
  </owl:DatatypeProperty>
  <owl:DatatypeProperty rdf:about="http://example.org/onto/prop/google_data_catalog_entry_sample_gcs_file_specs">
    <rdfs:label>sample_gcs_file_specs</rdfs:label>
    <rdfs:comment>Sample files contained in this fileset, not all files contained in this fileset are represented here.</rdfs:comment>
    <rdfs:domain rdf:resource="http://example.org/onto/class/google_data_catalog_entry"/>
    <rdfs:range rdf:resource="http://www.w3.org/2001/XMLSchema#string"/>
  </owl:DatatypeProperty>
  <owl:DatatypeProperty rdf:about="http://example.org/onto/prop/google_data_catalog_entry_create">
    <rdfs:label>create</rdfs:label>
    <rdfs:domain rdf:resource="http://example.org/onto/class/google_data_catalog_entry"/>
    <rdfs:range rdf:resource="http://www.w3.org/2001/XMLSchema#string"/>
  </owl:DatatypeProperty>
  <owl:DatatypeProperty rdf:about="http://example.org/onto/prop/google_data_catalog_entry_delete">
    <rdfs:label>delete</rdfs:label>
    <rdfs:domain rdf:resource="http://example.org/onto/class/google_data_catalog_entry"/>
    <rdfs:range rdf:resource="http://www.w3.org/2001/XMLSchema#string"/>
  </owl:DatatypeProperty>
  <owl:DatatypeProperty rdf:about="http://example.org/onto/prop/google_data_catalog_entry_update">
    <rdfs:label>update</rdfs:label>
    <rdfs:domain rdf:resource="http://example.org/onto/class/google_data_catalog_entry"/>
    <rdfs:range rdf:resource="http://www.w3.org/2001/XMLSchema#string"/>
  </owl:DatatypeProperty>
</rdf:RDF>
