<?xml version="1.0" encoding="UTF-8"?>
<rdf:RDF
  xmlns:rdf="http://www.w3.org/1999/02/22-rdf-syntax-ns#"
  xmlns:rdfs="http://www.w3.org/2000/01/rdf-schema#"
  xmlns:owl="http://www.w3.org/2002/07/owl#"
  xmlns:xsd="http://www.w3.org/2001/XMLSchema#"
  xml:base="http://example.org/onto/">
  <owl:Class rdf:about="http://example.org/onto/class/google_compute_region_url_map">
    <rdfs:label>google_compute_region_url_map</rdfs:label>
    <rdfs:comment>#
#     ***     AUTO GENERATED CODE    ***    Type: MMv1     ***
#
# ----------------------------------------------------------------------------
#
#     This code is generated by Magic Modules using the following:
#
#     Configuration: https:#github.com/GoogleCloudPlatform/magic-modules/tree/main/mmv1/products/compute/RegionUrlMap.yaml
#     Template:      https:#github.com/GoogleCloudPlatform/magic-modules/tree/main/mmv1/templates/terraform/resource.html.markdown.tmpl
#
#     DO NOT EDIT this file directly. Any changes made to this file will be
#     overwritten during the next generation cycle.
#
# ----------------------------------------------------------------------------
subcategory: "Compute Engine"
description: |-
  UrlMaps are used to route requests to a backend service based on rules
  that you define for the host and path of an incoming URL.
---</rdfs:comment>
  </owl:Class>
  <owl:DatatypeProperty rdf:about="http://example.org/onto/prop/google_compute_region_url_map_creation_timestamp">
    <rdfs:label>creation_timestamp</rdfs:label>
    <rdfs:comment>Creation timestamp in RFC3339 text format.</rdfs:comment>
    <rdfs:domain rdf:resource="http://example.org/onto/class/google_compute_region_url_map"/>
    <rdfs:range rdf:resource="http://www.w3.org/2001/XMLSchema#string"/>
  </owl:DatatypeProperty>
  <owl:DatatypeProperty rdf:about="http://example.org/onto/prop/google_compute_region_url_map_default_service">
    <rdfs:label>default_service</rdfs:label>
    <rdfs:comment>The full or partial URL of the defaultService resource to which traffic is directed if
none of the hostRules match. If defaultRouteAction is additionally specified, advanced
routing actions like URL Rewrites, etc. take effect prior to sending the request to the
backend. However, if defaultService is specified, defaultRouteAction cannot contain any
weightedBackendServices. Conversely, if routeAction specifies any
weightedBackendServices, service must not be specified.  Only one of defaultService,
defaultUrlRedirect or defaultRouteAction.weightedBackendService must be set.</rdfs:comment>
    <rdfs:domain rdf:resource="http://example.org/onto/class/google_compute_region_url_map"/>
    <rdfs:range rdf:resource="http://www.w3.org/2001/XMLSchema#string"/>
  </owl:DatatypeProperty>
  <owl:DatatypeProperty rdf:about="http://example.org/onto/prop/google_compute_region_url_map_description">
    <rdfs:label>description</rdfs:label>
    <rdfs:comment>An optional description of this resource. Provide this property when
you create the resource.</rdfs:comment>
    <rdfs:domain rdf:resource="http://example.org/onto/class/google_compute_region_url_map"/>
    <rdfs:range rdf:resource="http://www.w3.org/2001/XMLSchema#string"/>
  </owl:DatatypeProperty>
  <owl:DatatypeProperty rdf:about="http://example.org/onto/prop/google_compute_region_url_map_fingerprint">
    <rdfs:label>fingerprint</rdfs:label>
    <rdfs:comment>Fingerprint of this resource. This field is used internally during
updates of this resource.</rdfs:comment>
    <rdfs:domain rdf:resource="http://example.org/onto/class/google_compute_region_url_map"/>
    <rdfs:range rdf:resource="http://www.w3.org/2001/XMLSchema#string"/>
  </owl:DatatypeProperty>
  <owl:DatatypeProperty rdf:about="http://example.org/onto/prop/google_compute_region_url_map_id">
    <rdfs:label>id</rdfs:label>
    <rdfs:domain rdf:resource="http://example.org/onto/class/google_compute_region_url_map"/>
    <rdfs:range rdf:resource="http://www.w3.org/2001/XMLSchema#string"/>
  </owl:DatatypeProperty>
  <owl:DatatypeProperty rdf:about="http://example.org/onto/prop/google_compute_region_url_map_map_id">
    <rdfs:label>map_id</rdfs:label>
    <rdfs:comment>The unique identifier for the resource.</rdfs:comment>
    <rdfs:domain rdf:resource="http://example.org/onto/class/google_compute_region_url_map"/>
    <rdfs:range rdf:resource="http://www.w3.org/2001/XMLSchema#string"/>
  </owl:DatatypeProperty>
  <owl:DatatypeProperty rdf:about="http://example.org/onto/prop/google_compute_region_url_map_name">
    <rdfs:label>name</rdfs:label>
    <rdfs:comment>Name of the resource. Provided by the client when the resource is
created. The name must be 1-63 characters long, and comply with
RFC1035. Specifically, the name must be 1-63 characters long and match
the regular expression '[a-z]([-a-z0-9]*[a-z0-9])?' which means the
first character must be a lowercase letter, and all following
characters must be a dash, lowercase letter, or digit, except the last
character, which cannot be a dash.</rdfs:comment>
    <rdfs:domain rdf:resource="http://example.org/onto/class/google_compute_region_url_map"/>
    <rdfs:range rdf:resource="http://www.w3.org/2001/XMLSchema#string"/>
  </owl:DatatypeProperty>
  <owl:DatatypeProperty rdf:about="http://example.org/onto/prop/google_compute_region_url_map_project">
    <rdfs:label>project</rdfs:label>
    <rdfs:domain rdf:resource="http://example.org/onto/class/google_compute_region_url_map"/>
    <rdfs:range rdf:resource="http://www.w3.org/2001/XMLSchema#string"/>
  </owl:DatatypeProperty>
  <owl:DatatypeProperty rdf:about="http://example.org/onto/prop/google_compute_region_url_map_region">
    <rdfs:label>region</rdfs:label>
    <rdfs:comment>The Region in which the url map should reside.
If it is not provided, the provider region is used.</rdfs:comment>
    <rdfs:domain rdf:resource="http://example.org/onto/class/google_compute_region_url_map"/>
    <rdfs:range rdf:resource="http://www.w3.org/2001/XMLSchema#string"/>
  </owl:DatatypeProperty>
  <owl:DatatypeProperty rdf:about="http://example.org/onto/prop/google_compute_region_url_map_self_link">
    <rdfs:label>self_link</rdfs:label>
    <rdfs:domain rdf:resource="http://example.org/onto/class/google_compute_region_url_map"/>
    <rdfs:range rdf:resource="http://www.w3.org/2001/XMLSchema#string"/>
  </owl:DatatypeProperty>
  <owl:DatatypeProperty rdf:about="http://example.org/onto/prop/google_compute_region_url_map_allow_credentials">
    <rdfs:label>allow_credentials</rdfs:label>
    <rdfs:comment>In response to a preflight request, setting this to true indicates that the actual request can include user credentials. This field translates to the Access-Control-Allow-Credentials header.
Default is false.</rdfs:comment>
    <rdfs:domain rdf:resource="http://example.org/onto/class/google_compute_region_url_map"/>
    <rdfs:range rdf:resource="http://www.w3.org/2001/XMLSchema#string"/>
  </owl:DatatypeProperty>
  <owl:DatatypeProperty rdf:about="http://example.org/onto/prop/google_compute_region_url_map_allow_headers">
    <rdfs:label>allow_headers</rdfs:label>
    <rdfs:comment>Specifies the content for the Access-Control-Allow-Headers header.</rdfs:comment>
    <rdfs:domain rdf:resource="http://example.org/onto/class/google_compute_region_url_map"/>
    <rdfs:range rdf:resource="http://www.w3.org/2001/XMLSchema#string"/>
  </owl:DatatypeProperty>
  <owl:DatatypeProperty rdf:about="http://example.org/onto/prop/google_compute_region_url_map_allow_methods">
    <rdfs:label>allow_methods</rdfs:label>
    <rdfs:comment>Specifies the content for the Access-Control-Allow-Methods header.</rdfs:comment>
    <rdfs:domain rdf:resource="http://example.org/onto/class/google_compute_region_url_map"/>
    <rdfs:range rdf:resource="http://www.w3.org/2001/XMLSchema#string"/>
  </owl:DatatypeProperty>
  <owl:DatatypeProperty rdf:about="http://example.org/onto/prop/google_compute_region_url_map_allow_origin_regexes">
    <rdfs:label>allow_origin_regexes</rdfs:label>
    <rdfs:comment>Specifies the regualar expression patterns that match allowed origins. For regular expression grammar
please see en.cppreference.com/w/cpp/regex/ecmascript
An origin is allowed if it matches either an item in allowOrigins or an item in allowOriginRegexes.</rdfs:comment>
    <rdfs:domain rdf:resource="http://example.org/onto/class/google_compute_region_url_map"/>
    <rdfs:range rdf:resource="http://www.w3.org/2001/XMLSchema#string"/>
  </owl:DatatypeProperty>
  <owl:DatatypeProperty rdf:about="http://example.org/onto/prop/google_compute_region_url_map_allow_origins">
    <rdfs:label>allow_origins</rdfs:label>
    <rdfs:comment>Specifies the list of origins that will be allowed to do CORS requests.
An origin is allowed if it matches either an item in allowOrigins or an item in allowOriginRegexes.</rdfs:comment>
    <rdfs:domain rdf:resource="http://example.org/onto/class/google_compute_region_url_map"/>
    <rdfs:range rdf:resource="http://www.w3.org/2001/XMLSchema#string"/>
  </owl:DatatypeProperty>
  <owl:DatatypeProperty rdf:about="http://example.org/onto/prop/google_compute_region_url_map_disabled">
    <rdfs:label>disabled</rdfs:label>
    <rdfs:comment>If true, the setting specifies the CORS policy is disabled. The default value of false, which indicates that the CORS policy is in effect.</rdfs:comment>
    <rdfs:domain rdf:resource="http://example.org/onto/class/google_compute_region_url_map"/>
    <rdfs:range rdf:resource="http://www.w3.org/2001/XMLSchema#string"/>
  </owl:DatatypeProperty>
  <owl:DatatypeProperty rdf:about="http://example.org/onto/prop/google_compute_region_url_map_expose_headers">
    <rdfs:label>expose_headers</rdfs:label>
    <rdfs:comment>Specifies the content for the Access-Control-Expose-Headers header.</rdfs:comment>
    <rdfs:domain rdf:resource="http://example.org/onto/class/google_compute_region_url_map"/>
    <rdfs:range rdf:resource="http://www.w3.org/2001/XMLSchema#string"/>
  </owl:DatatypeProperty>
  <owl:DatatypeProperty rdf:about="http://example.org/onto/prop/google_compute_region_url_map_max_age">
    <rdfs:label>max_age</rdfs:label>
    <rdfs:comment>Specifies how long results of a preflight request can be cached in seconds.
This translates to the Access-Control-Max-Age header.</rdfs:comment>
    <rdfs:domain rdf:resource="http://example.org/onto/class/google_compute_region_url_map"/>
    <rdfs:range rdf:resource="http://www.w3.org/2001/XMLSchema#string"/>
  </owl:DatatypeProperty>
  <owl:DatatypeProperty rdf:about="http://example.org/onto/prop/google_compute_region_url_map_http_status">
    <rdfs:label>http_status</rdfs:label>
    <rdfs:comment>The HTTP status code used to abort the request.
The value must be between 200 and 599 inclusive.</rdfs:comment>
    <rdfs:domain rdf:resource="http://example.org/onto/class/google_compute_region_url_map"/>
    <rdfs:range rdf:resource="http://www.w3.org/2001/XMLSchema#string"/>
  </owl:DatatypeProperty>
  <owl:DatatypeProperty rdf:about="http://example.org/onto/prop/google_compute_region_url_map_percentage">
    <rdfs:label>percentage</rdfs:label>
    <rdfs:comment>The percentage of traffic (connections/operations/requests) which will be aborted as part of fault injection.
The value must be between 0.0 and 100.0 inclusive.</rdfs:comment>
    <rdfs:domain rdf:resource="http://example.org/onto/class/google_compute_region_url_map"/>
    <rdfs:range rdf:resource="http://www.w3.org/2001/XMLSchema#string"/>
  </owl:DatatypeProperty>
  <owl:DatatypeProperty rdf:about="http://example.org/onto/prop/google_compute_region_url_map_percentage">
    <rdfs:label>percentage</rdfs:label>
    <rdfs:comment>The percentage of traffic (connections/operations/requests) on which delay will be introduced as part of fault injection.
The value must be between 0.0 and 100.0 inclusive.</rdfs:comment>
    <rdfs:domain rdf:resource="http://example.org/onto/class/google_compute_region_url_map"/>
    <rdfs:range rdf:resource="http://www.w3.org/2001/XMLSchema#string"/>
  </owl:DatatypeProperty>
  <owl:DatatypeProperty rdf:about="http://example.org/onto/prop/google_compute_region_url_map_nanos">
    <rdfs:label>nanos</rdfs:label>
    <rdfs:comment>Span of time that's a fraction of a second at nanosecond resolution. Durations less than one second are
represented with a 0 seconds field and a positive nanos field. Must be from 0 to 999,999,999 inclusive.</rdfs:comment>
    <rdfs:domain rdf:resource="http://example.org/onto/class/google_compute_region_url_map"/>
    <rdfs:range rdf:resource="http://www.w3.org/2001/XMLSchema#string"/>
  </owl:DatatypeProperty>
  <owl:DatatypeProperty rdf:about="http://example.org/onto/prop/google_compute_region_url_map_seconds">
    <rdfs:label>seconds</rdfs:label>
    <rdfs:comment>Span of time at a resolution of a second. Must be from 0 to 315,576,000,000 inclusive.
Note: these bounds are computed from: 60 sec/min * 60 min/hr * 24 hr/day * 365.25 days/year * 10000 years</rdfs:comment>
    <rdfs:domain rdf:resource="http://example.org/onto/class/google_compute_region_url_map"/>
    <rdfs:range rdf:resource="http://www.w3.org/2001/XMLSchema#string"/>
  </owl:DatatypeProperty>
  <owl:DatatypeProperty rdf:about="http://example.org/onto/prop/google_compute_region_url_map_backend_service">
    <rdfs:label>backend_service</rdfs:label>
    <rdfs:comment>The full or partial URL to the RegionBackendService resource being mirrored to.
The backend service configured for a mirroring policy must reference backends that are of the same type as the original backend service matched in the URL map.
Serverless NEG backends are not currently supported as a mirrored backend service.</rdfs:comment>
    <rdfs:domain rdf:resource="http://example.org/onto/class/google_compute_region_url_map"/>
    <rdfs:range rdf:resource="http://www.w3.org/2001/XMLSchema#string"/>
  </owl:DatatypeProperty>
  <owl:DatatypeProperty rdf:about="http://example.org/onto/prop/google_compute_region_url_map_num_retries">
    <rdfs:label>num_retries</rdfs:label>
    <rdfs:comment>Specifies the allowed number retries. This number must be > 0. If not specified, defaults to 1.</rdfs:comment>
    <rdfs:domain rdf:resource="http://example.org/onto/class/google_compute_region_url_map"/>
    <rdfs:range rdf:resource="http://www.w3.org/2001/XMLSchema#string"/>
  </owl:DatatypeProperty>
  <owl:DatatypeProperty rdf:about="http://example.org/onto/prop/google_compute_region_url_map_retry_conditions">
    <rdfs:label>retry_conditions</rdfs:label>
    <rdfs:comment>Specifies one or more conditions when this retry policy applies.
Valid values are listed below. Only the following codes are supported when the URL map is bound to target gRPC proxy that has validateForProxyless field set to true: cancelled, deadline-exceeded, internal, resource-exhausted, unavailable.
  - 5xx : retry is attempted if the instance or endpoint responds with any 5xx response code, or if the instance or endpoint does not respond at all. For example, disconnects, reset, read timeout, connection failure, and refused streams.
  - gateway-error : Similar to 5xx, but only applies to response codes 502, 503 or 504.
  - connect-failure : a retry is attempted on failures connecting to the instance or endpoint. For example, connection timeouts.
  - retriable-4xx : a retry is attempted if the instance or endpoint responds with a 4xx response code. The only error that you can retry is error code 409.
  - refused-stream : a retry is attempted if the instance or endpoint resets the stream with a REFUSED_STREAM error code. This reset type indicates that it is safe to retry.
  - cancelled : a retry is attempted if the gRPC status code in the response header is set to cancelled.
  - deadline-exceeded : a retry is attempted if the gRPC status code in the response header is set to deadline-exceeded.
  - internal :  a retry is attempted if the gRPC status code in the response header is set to internal.
  - resource-exhausted : a retry is attempted if the gRPC status code in the response header is set to resource-exhausted.
  - unavailable : a retry is attempted if the gRPC status code in the response header is set to unavailable.</rdfs:comment>
    <rdfs:domain rdf:resource="http://example.org/onto/class/google_compute_region_url_map"/>
    <rdfs:range rdf:resource="http://www.w3.org/2001/XMLSchema#string"/>
  </owl:DatatypeProperty>
  <owl:DatatypeProperty rdf:about="http://example.org/onto/prop/google_compute_region_url_map_nanos">
    <rdfs:label>nanos</rdfs:label>
    <rdfs:comment>Span of time that's a fraction of a second at nanosecond resolution. Durations less than one second are
represented with a 0 seconds field and a positive nanos field. Must be from 0 to 999,999,999 inclusive.</rdfs:comment>
    <rdfs:domain rdf:resource="http://example.org/onto/class/google_compute_region_url_map"/>
    <rdfs:range rdf:resource="http://www.w3.org/2001/XMLSchema#string"/>
  </owl:DatatypeProperty>
  <owl:DatatypeProperty rdf:about="http://example.org/onto/prop/google_compute_region_url_map_seconds">
    <rdfs:label>seconds</rdfs:label>
    <rdfs:comment>Span of time at a resolution of a second. Must be from 0 to 315,576,000,000 inclusive.
Note: these bounds are computed from: 60 sec/min * 60 min/hr * 24 hr/day * 365.25 days/year * 10000 years</rdfs:comment>
    <rdfs:domain rdf:resource="http://example.org/onto/class/google_compute_region_url_map"/>
    <rdfs:range rdf:resource="http://www.w3.org/2001/XMLSchema#string"/>
  </owl:DatatypeProperty>
  <owl:DatatypeProperty rdf:about="http://example.org/onto/prop/google_compute_region_url_map_nanos">
    <rdfs:label>nanos</rdfs:label>
    <rdfs:comment>Span of time that's a fraction of a second at nanosecond resolution. Durations less than one second are represented with a 0 seconds field and a positive nanos field. Must be from 0 to 999,999,999 inclusive.</rdfs:comment>
    <rdfs:domain rdf:resource="http://example.org/onto/class/google_compute_region_url_map"/>
    <rdfs:range rdf:resource="http://www.w3.org/2001/XMLSchema#string"/>
  </owl:DatatypeProperty>
  <owl:DatatypeProperty rdf:about="http://example.org/onto/prop/google_compute_region_url_map_seconds">
    <rdfs:label>seconds</rdfs:label>
    <rdfs:comment>Span of time at a resolution of a second. Must be from 0 to 315,576,000,000 inclusive. Note: these bounds are computed from: 60 sec/min * 60 min/hr * 24 hr/day * 365.25 days/year * 10000 years</rdfs:comment>
    <rdfs:domain rdf:resource="http://example.org/onto/class/google_compute_region_url_map"/>
    <rdfs:range rdf:resource="http://www.w3.org/2001/XMLSchema#string"/>
  </owl:DatatypeProperty>
  <owl:DatatypeProperty rdf:about="http://example.org/onto/prop/google_compute_region_url_map_host_rewrite">
    <rdfs:label>host_rewrite</rdfs:label>
    <rdfs:comment>Before forwarding the request to the selected service, the request's host header is replaced with contents of hostRewrite.
The value must be from 1 to 255 characters.</rdfs:comment>
    <rdfs:domain rdf:resource="http://example.org/onto/class/google_compute_region_url_map"/>
    <rdfs:range rdf:resource="http://www.w3.org/2001/XMLSchema#string"/>
  </owl:DatatypeProperty>
  <owl:DatatypeProperty rdf:about="http://example.org/onto/prop/google_compute_region_url_map_path_prefix_rewrite">
    <rdfs:label>path_prefix_rewrite</rdfs:label>
    <rdfs:comment>Before forwarding the request to the selected backend service, the matching portion of the request's path is replaced by pathPrefixRewrite.
The value must be from 1 to 1024 characters.</rdfs:comment>
    <rdfs:domain rdf:resource="http://example.org/onto/class/google_compute_region_url_map"/>
    <rdfs:range rdf:resource="http://www.w3.org/2001/XMLSchema#string"/>
  </owl:DatatypeProperty>
  <owl:DatatypeProperty rdf:about="http://example.org/onto/prop/google_compute_region_url_map_backend_service">
    <rdfs:label>backend_service</rdfs:label>
    <rdfs:comment>The full or partial URL to the default BackendService resource. Before forwarding the request to backendService, the load balancer applies any relevant headerActions specified as part of this backendServiceWeight.</rdfs:comment>
    <rdfs:domain rdf:resource="http://example.org/onto/class/google_compute_region_url_map"/>
    <rdfs:range rdf:resource="http://www.w3.org/2001/XMLSchema#string"/>
  </owl:DatatypeProperty>
  <owl:DatatypeProperty rdf:about="http://example.org/onto/prop/google_compute_region_url_map_weight">
    <rdfs:label>weight</rdfs:label>
    <rdfs:comment>Specifies the fraction of traffic sent to a backend service, computed as weight / (sum of all weightedBackendService weights in routeAction) .
The selection of a backend service is determined only for new traffic. Once a user's request has been directed to a backend service, subsequent requests are sent to the same backend service as determined by the backend service's session affinity policy.
The value must be from 0 to 1000.</rdfs:comment>
    <rdfs:domain rdf:resource="http://example.org/onto/class/google_compute_region_url_map"/>
    <rdfs:range rdf:resource="http://www.w3.org/2001/XMLSchema#string"/>
  </owl:DatatypeProperty>
  <owl:DatatypeProperty rdf:about="http://example.org/onto/prop/google_compute_region_url_map_request_headers_to_remove">
    <rdfs:label>request_headers_to_remove</rdfs:label>
    <rdfs:comment>A list of header names for headers that need to be removed from the request before forwarding the request to the backendService.</rdfs:comment>
    <rdfs:domain rdf:resource="http://example.org/onto/class/google_compute_region_url_map"/>
    <rdfs:range rdf:resource="http://www.w3.org/2001/XMLSchema#string"/>
  </owl:DatatypeProperty>
  <owl:DatatypeProperty rdf:about="http://example.org/onto/prop/google_compute_region_url_map_response_headers_to_remove">
    <rdfs:label>response_headers_to_remove</rdfs:label>
    <rdfs:comment>A list of header names for headers that need to be removed from the response before sending the response back to the client.</rdfs:comment>
    <rdfs:domain rdf:resource="http://example.org/onto/class/google_compute_region_url_map"/>
    <rdfs:range rdf:resource="http://www.w3.org/2001/XMLSchema#string"/>
  </owl:DatatypeProperty>
  <owl:DatatypeProperty rdf:about="http://example.org/onto/prop/google_compute_region_url_map_header_name">
    <rdfs:label>header_name</rdfs:label>
    <rdfs:comment>The name of the header.</rdfs:comment>
    <rdfs:domain rdf:resource="http://example.org/onto/class/google_compute_region_url_map"/>
    <rdfs:range rdf:resource="http://www.w3.org/2001/XMLSchema#string"/>
  </owl:DatatypeProperty>
  <owl:DatatypeProperty rdf:about="http://example.org/onto/prop/google_compute_region_url_map_header_value">
    <rdfs:label>header_value</rdfs:label>
    <rdfs:comment>The value of the header to add.</rdfs:comment>
    <rdfs:domain rdf:resource="http://example.org/onto/class/google_compute_region_url_map"/>
    <rdfs:range rdf:resource="http://www.w3.org/2001/XMLSchema#string"/>
  </owl:DatatypeProperty>
  <owl:DatatypeProperty rdf:about="http://example.org/onto/prop/google_compute_region_url_map_replace">
    <rdfs:label>replace</rdfs:label>
    <rdfs:comment>If false, headerValue is appended to any values that already exist for the header. If true, headerValue is set for the header, discarding any values that were set for that header.
The default value is false.</rdfs:comment>
    <rdfs:domain rdf:resource="http://example.org/onto/class/google_compute_region_url_map"/>
    <rdfs:range rdf:resource="http://www.w3.org/2001/XMLSchema#string"/>
  </owl:DatatypeProperty>
  <owl:DatatypeProperty rdf:about="http://example.org/onto/prop/google_compute_region_url_map_header_name">
    <rdfs:label>header_name</rdfs:label>
    <rdfs:comment>The name of the header.</rdfs:comment>
    <rdfs:domain rdf:resource="http://example.org/onto/class/google_compute_region_url_map"/>
    <rdfs:range rdf:resource="http://www.w3.org/2001/XMLSchema#string"/>
  </owl:DatatypeProperty>
  <owl:DatatypeProperty rdf:about="http://example.org/onto/prop/google_compute_region_url_map_header_value">
    <rdfs:label>header_value</rdfs:label>
    <rdfs:comment>The value of the header to add.</rdfs:comment>
    <rdfs:domain rdf:resource="http://example.org/onto/class/google_compute_region_url_map"/>
    <rdfs:range rdf:resource="http://www.w3.org/2001/XMLSchema#string"/>
  </owl:DatatypeProperty>
  <owl:DatatypeProperty rdf:about="http://example.org/onto/prop/google_compute_region_url_map_replace">
    <rdfs:label>replace</rdfs:label>
    <rdfs:comment>If false, headerValue is appended to any values that already exist for the header. If true, headerValue is set for the header, discarding any values that were set for that header.
The default value is false.</rdfs:comment>
    <rdfs:domain rdf:resource="http://example.org/onto/class/google_compute_region_url_map"/>
    <rdfs:range rdf:resource="http://www.w3.org/2001/XMLSchema#string"/>
  </owl:DatatypeProperty>
  <owl:DatatypeProperty rdf:about="http://example.org/onto/prop/google_compute_region_url_map_host_redirect">
    <rdfs:label>host_redirect</rdfs:label>
    <rdfs:comment>The host that will be used in the redirect response instead of the one that was
supplied in the request. The value must be between 1 and 255 characters.</rdfs:comment>
    <rdfs:domain rdf:resource="http://example.org/onto/class/google_compute_region_url_map"/>
    <rdfs:range rdf:resource="http://www.w3.org/2001/XMLSchema#string"/>
  </owl:DatatypeProperty>
  <owl:DatatypeProperty rdf:about="http://example.org/onto/prop/google_compute_region_url_map_https_redirect">
    <rdfs:label>https_redirect</rdfs:label>
    <rdfs:comment>If set to true, the URL scheme in the redirected request is set to https. If set to
false, the URL scheme of the redirected request will remain the same as that of the
request. This must only be set for UrlMaps used in TargetHttpProxys. Setting this
true for TargetHttpsProxy is not permitted. The default is set to false.</rdfs:comment>
    <rdfs:domain rdf:resource="http://example.org/onto/class/google_compute_region_url_map"/>
    <rdfs:range rdf:resource="http://www.w3.org/2001/XMLSchema#string"/>
  </owl:DatatypeProperty>
  <owl:DatatypeProperty rdf:about="http://example.org/onto/prop/google_compute_region_url_map_path_redirect">
    <rdfs:label>path_redirect</rdfs:label>
    <rdfs:comment>The path that will be used in the redirect response instead of the one that was
supplied in the request. pathRedirect cannot be supplied together with
prefixRedirect. Supply one alone or neither. If neither is supplied, the path of the
original request will be used for the redirect. The value must be between 1 and 1024
characters.</rdfs:comment>
    <rdfs:domain rdf:resource="http://example.org/onto/class/google_compute_region_url_map"/>
    <rdfs:range rdf:resource="http://www.w3.org/2001/XMLSchema#string"/>
  </owl:DatatypeProperty>
  <owl:DatatypeProperty rdf:about="http://example.org/onto/prop/google_compute_region_url_map_prefix_redirect">
    <rdfs:label>prefix_redirect</rdfs:label>
    <rdfs:comment>The prefix that replaces the prefixMatch specified in the HttpRouteRuleMatch,
retaining the remaining portion of the URL before redirecting the request.
prefixRedirect cannot be supplied together with pathRedirect. Supply one alone or
neither. If neither is supplied, the path of the original request will be used for
the redirect. The value must be between 1 and 1024 characters.</rdfs:comment>
    <rdfs:domain rdf:resource="http://example.org/onto/class/google_compute_region_url_map"/>
    <rdfs:range rdf:resource="http://www.w3.org/2001/XMLSchema#string"/>
  </owl:DatatypeProperty>
  <owl:DatatypeProperty rdf:about="http://example.org/onto/prop/google_compute_region_url_map_redirect_response_code">
    <rdfs:label>redirect_response_code</rdfs:label>
    <rdfs:comment>The HTTP Status code to use for this RedirectAction. Supported values are:

* MOVED_PERMANENTLY_DEFAULT, which is the default value and corresponds to 301.

* FOUND, which corresponds to 302.

* SEE_OTHER which corresponds to 303.

* TEMPORARY_REDIRECT, which corresponds to 307. In this case, the request method
will be retained.

* PERMANENT_REDIRECT, which corresponds to 308. In this case,
the request method will be retained. Possible values: ["FOUND", "MOVED_PERMANENTLY_DEFAULT", "PERMANENT_REDIRECT", "SEE_OTHER", "TEMPORARY_REDIRECT"]</rdfs:comment>
    <rdfs:domain rdf:resource="http://example.org/onto/class/google_compute_region_url_map"/>
    <rdfs:range rdf:resource="http://www.w3.org/2001/XMLSchema#string"/>
  </owl:DatatypeProperty>
  <owl:DatatypeProperty rdf:about="http://example.org/onto/prop/google_compute_region_url_map_strip_query">
    <rdfs:label>strip_query</rdfs:label>
    <rdfs:comment>If set to true, any accompanying query portion of the original URL is removed prior
to redirecting the request. If set to false, the query portion of the original URL is
retained.
 This field is required to ensure an empty block is not set. The normal default value is false.</rdfs:comment>
    <rdfs:domain rdf:resource="http://example.org/onto/class/google_compute_region_url_map"/>
    <rdfs:range rdf:resource="http://www.w3.org/2001/XMLSchema#string"/>
  </owl:DatatypeProperty>
  <owl:DatatypeProperty rdf:about="http://example.org/onto/prop/google_compute_region_url_map_request_headers_to_remove">
    <rdfs:label>request_headers_to_remove</rdfs:label>
    <rdfs:comment>A list of header names for headers that need to be removed from the request before forwarding the request to the backendService.</rdfs:comment>
    <rdfs:domain rdf:resource="http://example.org/onto/class/google_compute_region_url_map"/>
    <rdfs:range rdf:resource="http://www.w3.org/2001/XMLSchema#string"/>
  </owl:DatatypeProperty>
  <owl:DatatypeProperty rdf:about="http://example.org/onto/prop/google_compute_region_url_map_response_headers_to_remove">
    <rdfs:label>response_headers_to_remove</rdfs:label>
    <rdfs:comment>A list of header names for headers that need to be removed from the response before sending the response back to the client.</rdfs:comment>
    <rdfs:domain rdf:resource="http://example.org/onto/class/google_compute_region_url_map"/>
    <rdfs:range rdf:resource="http://www.w3.org/2001/XMLSchema#string"/>
  </owl:DatatypeProperty>
  <owl:DatatypeProperty rdf:about="http://example.org/onto/prop/google_compute_region_url_map_header_name">
    <rdfs:label>header_name</rdfs:label>
    <rdfs:comment>The name of the header.</rdfs:comment>
    <rdfs:domain rdf:resource="http://example.org/onto/class/google_compute_region_url_map"/>
    <rdfs:range rdf:resource="http://www.w3.org/2001/XMLSchema#string"/>
  </owl:DatatypeProperty>
  <owl:DatatypeProperty rdf:about="http://example.org/onto/prop/google_compute_region_url_map_header_value">
    <rdfs:label>header_value</rdfs:label>
    <rdfs:comment>The value of the header to add.</rdfs:comment>
    <rdfs:domain rdf:resource="http://example.org/onto/class/google_compute_region_url_map"/>
    <rdfs:range rdf:resource="http://www.w3.org/2001/XMLSchema#string"/>
  </owl:DatatypeProperty>
  <owl:DatatypeProperty rdf:about="http://example.org/onto/prop/google_compute_region_url_map_replace">
    <rdfs:label>replace</rdfs:label>
    <rdfs:comment>If false, headerValue is appended to any values that already exist for the header. If true, headerValue is set for the header, discarding any values that were set for that header.
The default value is false.</rdfs:comment>
    <rdfs:domain rdf:resource="http://example.org/onto/class/google_compute_region_url_map"/>
    <rdfs:range rdf:resource="http://www.w3.org/2001/XMLSchema#string"/>
  </owl:DatatypeProperty>
  <owl:DatatypeProperty rdf:about="http://example.org/onto/prop/google_compute_region_url_map_header_name">
    <rdfs:label>header_name</rdfs:label>
    <rdfs:comment>The name of the header.</rdfs:comment>
    <rdfs:domain rdf:resource="http://example.org/onto/class/google_compute_region_url_map"/>
    <rdfs:range rdf:resource="http://www.w3.org/2001/XMLSchema#string"/>
  </owl:DatatypeProperty>
  <owl:DatatypeProperty rdf:about="http://example.org/onto/prop/google_compute_region_url_map_header_value">
    <rdfs:label>header_value</rdfs:label>
    <rdfs:comment>The value of the header to add.</rdfs:comment>
    <rdfs:domain rdf:resource="http://example.org/onto/class/google_compute_region_url_map"/>
    <rdfs:range rdf:resource="http://www.w3.org/2001/XMLSchema#string"/>
  </owl:DatatypeProperty>
  <owl:DatatypeProperty rdf:about="http://example.org/onto/prop/google_compute_region_url_map_replace">
    <rdfs:label>replace</rdfs:label>
    <rdfs:comment>If false, headerValue is appended to any values that already exist for the header. If true, headerValue is set for the header, discarding any values that were set for that header.
The default value is false.</rdfs:comment>
    <rdfs:domain rdf:resource="http://example.org/onto/class/google_compute_region_url_map"/>
    <rdfs:range rdf:resource="http://www.w3.org/2001/XMLSchema#string"/>
  </owl:DatatypeProperty>
  <owl:DatatypeProperty rdf:about="http://example.org/onto/prop/google_compute_region_url_map_description">
    <rdfs:label>description</rdfs:label>
    <rdfs:comment>An optional description of this HostRule. Provide this property
when you create the resource.</rdfs:comment>
    <rdfs:domain rdf:resource="http://example.org/onto/class/google_compute_region_url_map"/>
    <rdfs:range rdf:resource="http://www.w3.org/2001/XMLSchema#string"/>
  </owl:DatatypeProperty>
  <owl:DatatypeProperty rdf:about="http://example.org/onto/prop/google_compute_region_url_map_hosts">
    <rdfs:label>hosts</rdfs:label>
    <rdfs:comment>The list of host patterns to match. They must be valid
hostnames, except * will match any string of ([a-z0-9-.]*). In
that case, * must be the first character and must be followed in
the pattern by either - or ..</rdfs:comment>
    <rdfs:domain rdf:resource="http://example.org/onto/class/google_compute_region_url_map"/>
    <rdfs:range rdf:resource="http://www.w3.org/2001/XMLSchema#string"/>
  </owl:DatatypeProperty>
  <owl:DatatypeProperty rdf:about="http://example.org/onto/prop/google_compute_region_url_map_path_matcher">
    <rdfs:label>path_matcher</rdfs:label>
    <rdfs:comment>The name of the PathMatcher to use to match the path portion of
the URL if the hostRule matches the URL's host portion.</rdfs:comment>
    <rdfs:domain rdf:resource="http://example.org/onto/class/google_compute_region_url_map"/>
    <rdfs:range rdf:resource="http://www.w3.org/2001/XMLSchema#string"/>
  </owl:DatatypeProperty>
  <owl:DatatypeProperty rdf:about="http://example.org/onto/prop/google_compute_region_url_map_default_service">
    <rdfs:label>default_service</rdfs:label>
    <rdfs:comment>A reference to a RegionBackendService resource. This will be used if
none of the pathRules defined by this PathMatcher is matched by
the URL's path portion.</rdfs:comment>
    <rdfs:domain rdf:resource="http://example.org/onto/class/google_compute_region_url_map"/>
    <rdfs:range rdf:resource="http://www.w3.org/2001/XMLSchema#string"/>
  </owl:DatatypeProperty>
  <owl:DatatypeProperty rdf:about="http://example.org/onto/prop/google_compute_region_url_map_description">
    <rdfs:label>description</rdfs:label>
    <rdfs:comment>An optional description of this resource.</rdfs:comment>
    <rdfs:domain rdf:resource="http://example.org/onto/class/google_compute_region_url_map"/>
    <rdfs:range rdf:resource="http://www.w3.org/2001/XMLSchema#string"/>
  </owl:DatatypeProperty>
  <owl:DatatypeProperty rdf:about="http://example.org/onto/prop/google_compute_region_url_map_name">
    <rdfs:label>name</rdfs:label>
    <rdfs:comment>The name to which this PathMatcher is referred by the HostRule.</rdfs:comment>
    <rdfs:domain rdf:resource="http://example.org/onto/class/google_compute_region_url_map"/>
    <rdfs:range rdf:resource="http://www.w3.org/2001/XMLSchema#string"/>
  </owl:DatatypeProperty>
  <owl:DatatypeProperty rdf:about="http://example.org/onto/prop/google_compute_region_url_map_allow_credentials">
    <rdfs:label>allow_credentials</rdfs:label>
    <rdfs:comment>In response to a preflight request, setting this to true indicates that the actual request can include user credentials.
This translates to the Access-Control-Allow-Credentials header.</rdfs:comment>
    <rdfs:domain rdf:resource="http://example.org/onto/class/google_compute_region_url_map"/>
    <rdfs:range rdf:resource="http://www.w3.org/2001/XMLSchema#string"/>
  </owl:DatatypeProperty>
  <owl:DatatypeProperty rdf:about="http://example.org/onto/prop/google_compute_region_url_map_allow_headers">
    <rdfs:label>allow_headers</rdfs:label>
    <rdfs:comment>Specifies the content for the Access-Control-Allow-Headers header.</rdfs:comment>
    <rdfs:domain rdf:resource="http://example.org/onto/class/google_compute_region_url_map"/>
    <rdfs:range rdf:resource="http://www.w3.org/2001/XMLSchema#string"/>
  </owl:DatatypeProperty>
  <owl:DatatypeProperty rdf:about="http://example.org/onto/prop/google_compute_region_url_map_allow_methods">
    <rdfs:label>allow_methods</rdfs:label>
    <rdfs:comment>Specifies the content for the Access-Control-Allow-Methods header.</rdfs:comment>
    <rdfs:domain rdf:resource="http://example.org/onto/class/google_compute_region_url_map"/>
    <rdfs:range rdf:resource="http://www.w3.org/2001/XMLSchema#string"/>
  </owl:DatatypeProperty>
  <owl:DatatypeProperty rdf:about="http://example.org/onto/prop/google_compute_region_url_map_allow_origin_regexes">
    <rdfs:label>allow_origin_regexes</rdfs:label>
    <rdfs:comment>Specifies the regular expression patterns that match allowed origins. For regular expression grammar
please see en.cppreference.com/w/cpp/regex/ecmascript
An origin is allowed if it matches either an item in allowOrigins or an item in allowOriginRegexes.</rdfs:comment>
    <rdfs:domain rdf:resource="http://example.org/onto/class/google_compute_region_url_map"/>
    <rdfs:range rdf:resource="http://www.w3.org/2001/XMLSchema#string"/>
  </owl:DatatypeProperty>
  <owl:DatatypeProperty rdf:about="http://example.org/onto/prop/google_compute_region_url_map_allow_origins">
    <rdfs:label>allow_origins</rdfs:label>
    <rdfs:comment>Specifies the list of origins that will be allowed to do CORS requests.
An origin is allowed if it matches either an item in allowOrigins or an item in allowOriginRegexes.</rdfs:comment>
    <rdfs:domain rdf:resource="http://example.org/onto/class/google_compute_region_url_map"/>
    <rdfs:range rdf:resource="http://www.w3.org/2001/XMLSchema#string"/>
  </owl:DatatypeProperty>
  <owl:DatatypeProperty rdf:about="http://example.org/onto/prop/google_compute_region_url_map_disabled">
    <rdfs:label>disabled</rdfs:label>
    <rdfs:comment>If true, specifies the CORS policy is disabled. The default value is false, which indicates that the CORS policy is in effect.</rdfs:comment>
    <rdfs:domain rdf:resource="http://example.org/onto/class/google_compute_region_url_map"/>
    <rdfs:range rdf:resource="http://www.w3.org/2001/XMLSchema#string"/>
  </owl:DatatypeProperty>
  <owl:DatatypeProperty rdf:about="http://example.org/onto/prop/google_compute_region_url_map_expose_headers">
    <rdfs:label>expose_headers</rdfs:label>
    <rdfs:comment>Specifies the content for the Access-Control-Expose-Headers header.</rdfs:comment>
    <rdfs:domain rdf:resource="http://example.org/onto/class/google_compute_region_url_map"/>
    <rdfs:range rdf:resource="http://www.w3.org/2001/XMLSchema#string"/>
  </owl:DatatypeProperty>
  <owl:DatatypeProperty rdf:about="http://example.org/onto/prop/google_compute_region_url_map_max_age">
    <rdfs:label>max_age</rdfs:label>
    <rdfs:comment>Specifies how long results of a preflight request can be cached in seconds.
This translates to the Access-Control-Max-Age header.</rdfs:comment>
    <rdfs:domain rdf:resource="http://example.org/onto/class/google_compute_region_url_map"/>
    <rdfs:range rdf:resource="http://www.w3.org/2001/XMLSchema#string"/>
  </owl:DatatypeProperty>
  <owl:DatatypeProperty rdf:about="http://example.org/onto/prop/google_compute_region_url_map_http_status">
    <rdfs:label>http_status</rdfs:label>
    <rdfs:comment>The HTTP status code used to abort the request.
The value must be between 200 and 599 inclusive.</rdfs:comment>
    <rdfs:domain rdf:resource="http://example.org/onto/class/google_compute_region_url_map"/>
    <rdfs:range rdf:resource="http://www.w3.org/2001/XMLSchema#string"/>
  </owl:DatatypeProperty>
  <owl:DatatypeProperty rdf:about="http://example.org/onto/prop/google_compute_region_url_map_percentage">
    <rdfs:label>percentage</rdfs:label>
    <rdfs:comment>The percentage of traffic (connections/operations/requests) which will be aborted as part of fault injection.
The value must be between 0.0 and 100.0 inclusive.</rdfs:comment>
    <rdfs:domain rdf:resource="http://example.org/onto/class/google_compute_region_url_map"/>
    <rdfs:range rdf:resource="http://www.w3.org/2001/XMLSchema#string"/>
  </owl:DatatypeProperty>
  <owl:DatatypeProperty rdf:about="http://example.org/onto/prop/google_compute_region_url_map_percentage">
    <rdfs:label>percentage</rdfs:label>
    <rdfs:comment>The percentage of traffic (connections/operations/requests) on which delay will be introduced as part of fault injection.
The value must be between 0.0 and 100.0 inclusive.</rdfs:comment>
    <rdfs:domain rdf:resource="http://example.org/onto/class/google_compute_region_url_map"/>
    <rdfs:range rdf:resource="http://www.w3.org/2001/XMLSchema#string"/>
  </owl:DatatypeProperty>
  <owl:DatatypeProperty rdf:about="http://example.org/onto/prop/google_compute_region_url_map_nanos">
    <rdfs:label>nanos</rdfs:label>
    <rdfs:comment>Span of time that's a fraction of a second at nanosecond resolution. Durations less than one second are
represented with a 0 seconds field and a positive nanos field. Must be from 0 to 999,999,999 inclusive.</rdfs:comment>
    <rdfs:domain rdf:resource="http://example.org/onto/class/google_compute_region_url_map"/>
    <rdfs:range rdf:resource="http://www.w3.org/2001/XMLSchema#string"/>
  </owl:DatatypeProperty>
  <owl:DatatypeProperty rdf:about="http://example.org/onto/prop/google_compute_region_url_map_seconds">
    <rdfs:label>seconds</rdfs:label>
    <rdfs:comment>Span of time at a resolution of a second. Must be from 0 to 315,576,000,000 inclusive.
Note: these bounds are computed from: 60 sec/min * 60 min/hr * 24 hr/day * 365.25 days/year * 10000 years</rdfs:comment>
    <rdfs:domain rdf:resource="http://example.org/onto/class/google_compute_region_url_map"/>
    <rdfs:range rdf:resource="http://www.w3.org/2001/XMLSchema#string"/>
  </owl:DatatypeProperty>
  <owl:DatatypeProperty rdf:about="http://example.org/onto/prop/google_compute_region_url_map_nanos">
    <rdfs:label>nanos</rdfs:label>
    <rdfs:comment>Span of time that's a fraction of a second at nanosecond resolution. Durations less than one second are represented
with a 0 seconds field and a positive nanos field. Must be from 0 to 999,999,999 inclusive.</rdfs:comment>
    <rdfs:domain rdf:resource="http://example.org/onto/class/google_compute_region_url_map"/>
    <rdfs:range rdf:resource="http://www.w3.org/2001/XMLSchema#string"/>
  </owl:DatatypeProperty>
  <owl:DatatypeProperty rdf:about="http://example.org/onto/prop/google_compute_region_url_map_seconds">
    <rdfs:label>seconds</rdfs:label>
    <rdfs:comment>Span of time at a resolution of a second. Must be from 0 to 315,576,000,000 inclusive.
Note: these bounds are computed from: 60 sec/min * 60 min/hr * 24 hr/day * 365.25 days/year * 10000 years</rdfs:comment>
    <rdfs:domain rdf:resource="http://example.org/onto/class/google_compute_region_url_map"/>
    <rdfs:range rdf:resource="http://www.w3.org/2001/XMLSchema#string"/>
  </owl:DatatypeProperty>
  <owl:DatatypeProperty rdf:about="http://example.org/onto/prop/google_compute_region_url_map_backend_service">
    <rdfs:label>backend_service</rdfs:label>
    <rdfs:comment>The full or partial URL to the BackendService resource being mirrored to.</rdfs:comment>
    <rdfs:domain rdf:resource="http://example.org/onto/class/google_compute_region_url_map"/>
    <rdfs:range rdf:resource="http://www.w3.org/2001/XMLSchema#string"/>
  </owl:DatatypeProperty>
  <owl:DatatypeProperty rdf:about="http://example.org/onto/prop/google_compute_region_url_map_num_retries">
    <rdfs:label>num_retries</rdfs:label>
    <rdfs:comment>Specifies the allowed number retries. This number must be > 0. If not specified, defaults to 1.</rdfs:comment>
    <rdfs:domain rdf:resource="http://example.org/onto/class/google_compute_region_url_map"/>
    <rdfs:range rdf:resource="http://www.w3.org/2001/XMLSchema#string"/>
  </owl:DatatypeProperty>
  <owl:DatatypeProperty rdf:about="http://example.org/onto/prop/google_compute_region_url_map_retry_conditions">
    <rdfs:label>retry_conditions</rdfs:label>
    <rdfs:comment>Specfies one or more conditions when this retry rule applies. Valid values are:

* 5xx: Loadbalancer will attempt a retry if the backend service responds with any 5xx response code,
  or if the backend service does not respond at all, example: disconnects, reset, read timeout,
* connection failure, and refused streams.
* gateway-error: Similar to 5xx, but only applies to response codes 502, 503 or 504.
* connect-failure: Loadbalancer will retry on failures connecting to backend services,
  for example due to connection timeouts.
* retriable-4xx: Loadbalancer will retry for retriable 4xx response codes.
  Currently the only retriable error supported is 409.
* refused-stream:Loadbalancer will retry if the backend service resets the stream with a REFUSED_STREAM error code.
  This reset type indicates that it is safe to retry.
* cancelled: Loadbalancer will retry if the gRPC status code in the response header is set to cancelled
* deadline-exceeded: Loadbalancer will retry if the gRPC status code in the response header is set to deadline-exceeded
* resource-exhausted: Loadbalancer will retry if the gRPC status code in the response header is set to resource-exhausted
* unavailable: Loadbalancer will retry if the gRPC status code in the response header is set to unavailable</rdfs:comment>
    <rdfs:domain rdf:resource="http://example.org/onto/class/google_compute_region_url_map"/>
    <rdfs:range rdf:resource="http://www.w3.org/2001/XMLSchema#string"/>
  </owl:DatatypeProperty>
  <owl:DatatypeProperty rdf:about="http://example.org/onto/prop/google_compute_region_url_map_nanos">
    <rdfs:label>nanos</rdfs:label>
    <rdfs:comment>Span of time that's a fraction of a second at nanosecond resolution. Durations less than one second are
represented with a 0 seconds field and a positive nanos field. Must be from 0 to 999,999,999 inclusive.</rdfs:comment>
    <rdfs:domain rdf:resource="http://example.org/onto/class/google_compute_region_url_map"/>
    <rdfs:range rdf:resource="http://www.w3.org/2001/XMLSchema#string"/>
  </owl:DatatypeProperty>
  <owl:DatatypeProperty rdf:about="http://example.org/onto/prop/google_compute_region_url_map_seconds">
    <rdfs:label>seconds</rdfs:label>
    <rdfs:comment>Span of time at a resolution of a second. Must be from 0 to 315,576,000,000 inclusive.
Note: these bounds are computed from: 60 sec/min * 60 min/hr * 24 hr/day * 365.25 days/year * 10000 years</rdfs:comment>
    <rdfs:domain rdf:resource="http://example.org/onto/class/google_compute_region_url_map"/>
    <rdfs:range rdf:resource="http://www.w3.org/2001/XMLSchema#string"/>
  </owl:DatatypeProperty>
  <owl:DatatypeProperty rdf:about="http://example.org/onto/prop/google_compute_region_url_map_nanos">
    <rdfs:label>nanos</rdfs:label>
    <rdfs:comment>Span of time that's a fraction of a second at nanosecond resolution. Durations less than one second are represented
with a 0 seconds field and a positive nanos field. Must be from 0 to 999,999,999 inclusive.</rdfs:comment>
    <rdfs:domain rdf:resource="http://example.org/onto/class/google_compute_region_url_map"/>
    <rdfs:range rdf:resource="http://www.w3.org/2001/XMLSchema#string"/>
  </owl:DatatypeProperty>
  <owl:DatatypeProperty rdf:about="http://example.org/onto/prop/google_compute_region_url_map_seconds">
    <rdfs:label>seconds</rdfs:label>
    <rdfs:comment>Span of time at a resolution of a second. Must be from 0 to 315,576,000,000 inclusive.
Note: these bounds are computed from: 60 sec/min * 60 min/hr * 24 hr/day * 365.25 days/year * 10000 years</rdfs:comment>
    <rdfs:domain rdf:resource="http://example.org/onto/class/google_compute_region_url_map"/>
    <rdfs:range rdf:resource="http://www.w3.org/2001/XMLSchema#string"/>
  </owl:DatatypeProperty>
  <owl:DatatypeProperty rdf:about="http://example.org/onto/prop/google_compute_region_url_map_host_rewrite">
    <rdfs:label>host_rewrite</rdfs:label>
    <rdfs:comment>Prior to forwarding the request to the selected service, the request's host header is replaced
with contents of hostRewrite.

The value must be between 1 and 255 characters.</rdfs:comment>
    <rdfs:domain rdf:resource="http://example.org/onto/class/google_compute_region_url_map"/>
    <rdfs:range rdf:resource="http://www.w3.org/2001/XMLSchema#string"/>
  </owl:DatatypeProperty>
  <owl:DatatypeProperty rdf:about="http://example.org/onto/prop/google_compute_region_url_map_path_prefix_rewrite">
    <rdfs:label>path_prefix_rewrite</rdfs:label>
    <rdfs:comment>Prior to forwarding the request to the selected backend service, the matching portion of the
request's path is replaced by pathPrefixRewrite.

The value must be between 1 and 1024 characters.</rdfs:comment>
    <rdfs:domain rdf:resource="http://example.org/onto/class/google_compute_region_url_map"/>
    <rdfs:range rdf:resource="http://www.w3.org/2001/XMLSchema#string"/>
  </owl:DatatypeProperty>
  <owl:DatatypeProperty rdf:about="http://example.org/onto/prop/google_compute_region_url_map_path_template_rewrite">
    <rdfs:label>path_template_rewrite</rdfs:label>
    <rdfs:comment>If specified, the pattern rewrites the URL path (based on the :path header) using the HTTP template syntax.

A corresponding pathTemplateMatch must be specified. Any template variables must exist in the pathTemplateMatch field.

* At least one variable must be specified in the pathTemplateMatch field
* You can omit variables from the rewritten URL
* The * and ** operators cannot be matched unless they have a corresponding variable name - e.g. {format=*} or {var=**}.

For example, a pathTemplateMatch of /static/{format=**} could be rewritten as /static/content/{format} to prefix
/content to the URL. Variables can also be re-ordered in a rewrite, so that /{country}/{format}/{suffix=**} can be
rewritten as /content/{format}/{country}/{suffix}.

At least one non-empty routeRules[].matchRules[].path_template_match is required.

Only one of pathPrefixRewrite or pathTemplateRewrite may be specified.</rdfs:comment>
    <rdfs:domain rdf:resource="http://example.org/onto/class/google_compute_region_url_map"/>
    <rdfs:range rdf:resource="http://www.w3.org/2001/XMLSchema#string"/>
  </owl:DatatypeProperty>
  <owl:DatatypeProperty rdf:about="http://example.org/onto/prop/google_compute_region_url_map_backend_service">
    <rdfs:label>backend_service</rdfs:label>
    <rdfs:comment>The full or partial URL to the default BackendService resource. Before forwarding the
request to backendService, the loadbalancer applies any relevant headerActions
specified as part of this backendServiceWeight.</rdfs:comment>
    <rdfs:domain rdf:resource="http://example.org/onto/class/google_compute_region_url_map"/>
    <rdfs:range rdf:resource="http://www.w3.org/2001/XMLSchema#string"/>
  </owl:DatatypeProperty>
  <owl:DatatypeProperty rdf:about="http://example.org/onto/prop/google_compute_region_url_map_weight">
    <rdfs:label>weight</rdfs:label>
    <rdfs:comment>Specifies the fraction of traffic sent to backendService, computed as
weight / (sum of all weightedBackendService weights in routeAction) .

The selection of a backend service is determined only for new traffic. Once a user's request
has been directed to a backendService, subsequent requests will be sent to the same backendService
as determined by the BackendService's session affinity policy.

The value must be between 0 and 1000</rdfs:comment>
    <rdfs:domain rdf:resource="http://example.org/onto/class/google_compute_region_url_map"/>
    <rdfs:range rdf:resource="http://www.w3.org/2001/XMLSchema#string"/>
  </owl:DatatypeProperty>
  <owl:DatatypeProperty rdf:about="http://example.org/onto/prop/google_compute_region_url_map_request_headers_to_remove">
    <rdfs:label>request_headers_to_remove</rdfs:label>
    <rdfs:comment>A list of header names for headers that need to be removed from the request prior to
forwarding the request to the backendService.</rdfs:comment>
    <rdfs:domain rdf:resource="http://example.org/onto/class/google_compute_region_url_map"/>
    <rdfs:range rdf:resource="http://www.w3.org/2001/XMLSchema#string"/>
  </owl:DatatypeProperty>
  <owl:DatatypeProperty rdf:about="http://example.org/onto/prop/google_compute_region_url_map_response_headers_to_remove">
    <rdfs:label>response_headers_to_remove</rdfs:label>
    <rdfs:comment>A list of header names for headers that need to be removed from the response prior to sending the
response back to the client.</rdfs:comment>
    <rdfs:domain rdf:resource="http://example.org/onto/class/google_compute_region_url_map"/>
    <rdfs:range rdf:resource="http://www.w3.org/2001/XMLSchema#string"/>
  </owl:DatatypeProperty>
  <owl:DatatypeProperty rdf:about="http://example.org/onto/prop/google_compute_region_url_map_header_name">
    <rdfs:label>header_name</rdfs:label>
    <rdfs:comment>The name of the header to add.</rdfs:comment>
    <rdfs:domain rdf:resource="http://example.org/onto/class/google_compute_region_url_map"/>
    <rdfs:range rdf:resource="http://www.w3.org/2001/XMLSchema#string"/>
  </owl:DatatypeProperty>
  <owl:DatatypeProperty rdf:about="http://example.org/onto/prop/google_compute_region_url_map_header_value">
    <rdfs:label>header_value</rdfs:label>
    <rdfs:comment>The value of the header to add.</rdfs:comment>
    <rdfs:domain rdf:resource="http://example.org/onto/class/google_compute_region_url_map"/>
    <rdfs:range rdf:resource="http://www.w3.org/2001/XMLSchema#string"/>
  </owl:DatatypeProperty>
  <owl:DatatypeProperty rdf:about="http://example.org/onto/prop/google_compute_region_url_map_replace">
    <rdfs:label>replace</rdfs:label>
    <rdfs:comment>If false, headerValue is appended to any values that already exist for the header.
If true, headerValue is set for the header, discarding any values that were set for that header.</rdfs:comment>
    <rdfs:domain rdf:resource="http://example.org/onto/class/google_compute_region_url_map"/>
    <rdfs:range rdf:resource="http://www.w3.org/2001/XMLSchema#string"/>
  </owl:DatatypeProperty>
  <owl:DatatypeProperty rdf:about="http://example.org/onto/prop/google_compute_region_url_map_header_name">
    <rdfs:label>header_name</rdfs:label>
    <rdfs:comment>The name of the header to add.</rdfs:comment>
    <rdfs:domain rdf:resource="http://example.org/onto/class/google_compute_region_url_map"/>
    <rdfs:range rdf:resource="http://www.w3.org/2001/XMLSchema#string"/>
  </owl:DatatypeProperty>
  <owl:DatatypeProperty rdf:about="http://example.org/onto/prop/google_compute_region_url_map_header_value">
    <rdfs:label>header_value</rdfs:label>
    <rdfs:comment>The value of the header to add.</rdfs:comment>
    <rdfs:domain rdf:resource="http://example.org/onto/class/google_compute_region_url_map"/>
    <rdfs:range rdf:resource="http://www.w3.org/2001/XMLSchema#string"/>
  </owl:DatatypeProperty>
  <owl:DatatypeProperty rdf:about="http://example.org/onto/prop/google_compute_region_url_map_replace">
    <rdfs:label>replace</rdfs:label>
    <rdfs:comment>If false, headerValue is appended to any values that already exist for the header.
If true, headerValue is set for the header, discarding any values that were set for that header.</rdfs:comment>
    <rdfs:domain rdf:resource="http://example.org/onto/class/google_compute_region_url_map"/>
    <rdfs:range rdf:resource="http://www.w3.org/2001/XMLSchema#string"/>
  </owl:DatatypeProperty>
  <owl:DatatypeProperty rdf:about="http://example.org/onto/prop/google_compute_region_url_map_host_redirect">
    <rdfs:label>host_redirect</rdfs:label>
    <rdfs:comment>The host that will be used in the redirect response instead of the one that was
supplied in the request. The value must be between 1 and 255 characters.</rdfs:comment>
    <rdfs:domain rdf:resource="http://example.org/onto/class/google_compute_region_url_map"/>
    <rdfs:range rdf:resource="http://www.w3.org/2001/XMLSchema#string"/>
  </owl:DatatypeProperty>
  <owl:DatatypeProperty rdf:about="http://example.org/onto/prop/google_compute_region_url_map_https_redirect">
    <rdfs:label>https_redirect</rdfs:label>
    <rdfs:comment>If set to true, the URL scheme in the redirected request is set to https. If set to
false, the URL scheme of the redirected request will remain the same as that of the
request. This must only be set for UrlMaps used in TargetHttpProxys. Setting this
true for TargetHttpsProxy is not permitted. The default is set to false.</rdfs:comment>
    <rdfs:domain rdf:resource="http://example.org/onto/class/google_compute_region_url_map"/>
    <rdfs:range rdf:resource="http://www.w3.org/2001/XMLSchema#string"/>
  </owl:DatatypeProperty>
  <owl:DatatypeProperty rdf:about="http://example.org/onto/prop/google_compute_region_url_map_path_redirect">
    <rdfs:label>path_redirect</rdfs:label>
    <rdfs:comment>The path that will be used in the redirect response instead of the one that was
supplied in the request. pathRedirect cannot be supplied together with
prefixRedirect. Supply one alone or neither. If neither is supplied, the path of the
original request will be used for the redirect. The value must be between 1 and 1024
characters.</rdfs:comment>
    <rdfs:domain rdf:resource="http://example.org/onto/class/google_compute_region_url_map"/>
    <rdfs:range rdf:resource="http://www.w3.org/2001/XMLSchema#string"/>
  </owl:DatatypeProperty>
  <owl:DatatypeProperty rdf:about="http://example.org/onto/prop/google_compute_region_url_map_prefix_redirect">
    <rdfs:label>prefix_redirect</rdfs:label>
    <rdfs:comment>The prefix that replaces the prefixMatch specified in the HttpRouteRuleMatch,
retaining the remaining portion of the URL before redirecting the request.
prefixRedirect cannot be supplied together with pathRedirect. Supply one alone or
neither. If neither is supplied, the path of the original request will be used for
the redirect. The value must be between 1 and 1024 characters.</rdfs:comment>
    <rdfs:domain rdf:resource="http://example.org/onto/class/google_compute_region_url_map"/>
    <rdfs:range rdf:resource="http://www.w3.org/2001/XMLSchema#string"/>
  </owl:DatatypeProperty>
  <owl:DatatypeProperty rdf:about="http://example.org/onto/prop/google_compute_region_url_map_redirect_response_code">
    <rdfs:label>redirect_response_code</rdfs:label>
    <rdfs:comment>The HTTP Status code to use for this RedirectAction. Supported values are:

* MOVED_PERMANENTLY_DEFAULT, which is the default value and corresponds to 301.

* FOUND, which corresponds to 302.

* SEE_OTHER which corresponds to 303.

* TEMPORARY_REDIRECT, which corresponds to 307. In this case, the request method
will be retained.

* PERMANENT_REDIRECT, which corresponds to 308. In this case,
the request method will be retained. Possible values: ["FOUND", "MOVED_PERMANENTLY_DEFAULT", "PERMANENT_REDIRECT", "SEE_OTHER", "TEMPORARY_REDIRECT"]</rdfs:comment>
    <rdfs:domain rdf:resource="http://example.org/onto/class/google_compute_region_url_map"/>
    <rdfs:range rdf:resource="http://www.w3.org/2001/XMLSchema#string"/>
  </owl:DatatypeProperty>
  <owl:DatatypeProperty rdf:about="http://example.org/onto/prop/google_compute_region_url_map_strip_query">
    <rdfs:label>strip_query</rdfs:label>
    <rdfs:comment>If set to true, any accompanying query portion of the original URL is removed prior
to redirecting the request. If set to false, the query portion of the original URL is
retained.
 This field is required to ensure an empty block is not set. The normal default value is false.</rdfs:comment>
    <rdfs:domain rdf:resource="http://example.org/onto/class/google_compute_region_url_map"/>
    <rdfs:range rdf:resource="http://www.w3.org/2001/XMLSchema#string"/>
  </owl:DatatypeProperty>
  <owl:DatatypeProperty rdf:about="http://example.org/onto/prop/google_compute_region_url_map_request_headers_to_remove">
    <rdfs:label>request_headers_to_remove</rdfs:label>
    <rdfs:comment>A list of header names for headers that need to be removed from the request before forwarding the request to the backendService.</rdfs:comment>
    <rdfs:domain rdf:resource="http://example.org/onto/class/google_compute_region_url_map"/>
    <rdfs:range rdf:resource="http://www.w3.org/2001/XMLSchema#string"/>
  </owl:DatatypeProperty>
  <owl:DatatypeProperty rdf:about="http://example.org/onto/prop/google_compute_region_url_map_response_headers_to_remove">
    <rdfs:label>response_headers_to_remove</rdfs:label>
    <rdfs:comment>A list of header names for headers that need to be removed from the response before sending the response back to the client.</rdfs:comment>
    <rdfs:domain rdf:resource="http://example.org/onto/class/google_compute_region_url_map"/>
    <rdfs:range rdf:resource="http://www.w3.org/2001/XMLSchema#string"/>
  </owl:DatatypeProperty>
  <owl:DatatypeProperty rdf:about="http://example.org/onto/prop/google_compute_region_url_map_header_name">
    <rdfs:label>header_name</rdfs:label>
    <rdfs:comment>The name of the header.</rdfs:comment>
    <rdfs:domain rdf:resource="http://example.org/onto/class/google_compute_region_url_map"/>
    <rdfs:range rdf:resource="http://www.w3.org/2001/XMLSchema#string"/>
  </owl:DatatypeProperty>
  <owl:DatatypeProperty rdf:about="http://example.org/onto/prop/google_compute_region_url_map_header_value">
    <rdfs:label>header_value</rdfs:label>
    <rdfs:comment>The value of the header to add.</rdfs:comment>
    <rdfs:domain rdf:resource="http://example.org/onto/class/google_compute_region_url_map"/>
    <rdfs:range rdf:resource="http://www.w3.org/2001/XMLSchema#string"/>
  </owl:DatatypeProperty>
  <owl:DatatypeProperty rdf:about="http://example.org/onto/prop/google_compute_region_url_map_replace">
    <rdfs:label>replace</rdfs:label>
    <rdfs:comment>If false, headerValue is appended to any values that already exist for the header. If true, headerValue is set for the header, discarding any values that were set for that header.
The default value is false.</rdfs:comment>
    <rdfs:domain rdf:resource="http://example.org/onto/class/google_compute_region_url_map"/>
    <rdfs:range rdf:resource="http://www.w3.org/2001/XMLSchema#string"/>
  </owl:DatatypeProperty>
  <owl:DatatypeProperty rdf:about="http://example.org/onto/prop/google_compute_region_url_map_header_name">
    <rdfs:label>header_name</rdfs:label>
    <rdfs:comment>The name of the header.</rdfs:comment>
    <rdfs:domain rdf:resource="http://example.org/onto/class/google_compute_region_url_map"/>
    <rdfs:range rdf:resource="http://www.w3.org/2001/XMLSchema#string"/>
  </owl:DatatypeProperty>
  <owl:DatatypeProperty rdf:about="http://example.org/onto/prop/google_compute_region_url_map_header_value">
    <rdfs:label>header_value</rdfs:label>
    <rdfs:comment>The value of the header to add.</rdfs:comment>
    <rdfs:domain rdf:resource="http://example.org/onto/class/google_compute_region_url_map"/>
    <rdfs:range rdf:resource="http://www.w3.org/2001/XMLSchema#string"/>
  </owl:DatatypeProperty>
  <owl:DatatypeProperty rdf:about="http://example.org/onto/prop/google_compute_region_url_map_replace">
    <rdfs:label>replace</rdfs:label>
    <rdfs:comment>If false, headerValue is appended to any values that already exist for the header. If true, headerValue is set for the header, discarding any values that were set for that header.
The default value is false.</rdfs:comment>
    <rdfs:domain rdf:resource="http://example.org/onto/class/google_compute_region_url_map"/>
    <rdfs:range rdf:resource="http://www.w3.org/2001/XMLSchema#string"/>
  </owl:DatatypeProperty>
  <owl:DatatypeProperty rdf:about="http://example.org/onto/prop/google_compute_region_url_map_paths">
    <rdfs:label>paths</rdfs:label>
    <rdfs:comment>The list of path patterns to match. Each must start with / and the only place a
\* is allowed is at the end following a /. The string fed to the path matcher
does not include any text after the first ? or #, and those chars are not
allowed here.</rdfs:comment>
    <rdfs:domain rdf:resource="http://example.org/onto/class/google_compute_region_url_map"/>
    <rdfs:range rdf:resource="http://www.w3.org/2001/XMLSchema#string"/>
  </owl:DatatypeProperty>
  <owl:DatatypeProperty rdf:about="http://example.org/onto/prop/google_compute_region_url_map_service">
    <rdfs:label>service</rdfs:label>
    <rdfs:comment>The region backend service resource to which traffic is
directed if this rule is matched. If routeAction is additionally specified,
advanced routing actions like URL Rewrites, etc. take effect prior to sending
the request to the backend. However, if service is specified, routeAction cannot
contain any weightedBackendService s. Conversely, if routeAction specifies any
weightedBackendServices, service must not be specified. Only one of urlRedirect,
service or routeAction.weightedBackendService must be set.</rdfs:comment>
    <rdfs:domain rdf:resource="http://example.org/onto/class/google_compute_region_url_map"/>
    <rdfs:range rdf:resource="http://www.w3.org/2001/XMLSchema#string"/>
  </owl:DatatypeProperty>
  <owl:DatatypeProperty rdf:about="http://example.org/onto/prop/google_compute_region_url_map_allow_credentials">
    <rdfs:label>allow_credentials</rdfs:label>
    <rdfs:comment>In response to a preflight request, setting this to true indicates that the
actual request can include user credentials. This translates to the Access-
Control-Allow-Credentials header. Defaults to false.</rdfs:comment>
    <rdfs:domain rdf:resource="http://example.org/onto/class/google_compute_region_url_map"/>
    <rdfs:range rdf:resource="http://www.w3.org/2001/XMLSchema#string"/>
  </owl:DatatypeProperty>
  <owl:DatatypeProperty rdf:about="http://example.org/onto/prop/google_compute_region_url_map_allow_headers">
    <rdfs:label>allow_headers</rdfs:label>
    <rdfs:comment>Specifies the content for the Access-Control-Allow-Headers header.</rdfs:comment>
    <rdfs:domain rdf:resource="http://example.org/onto/class/google_compute_region_url_map"/>
    <rdfs:range rdf:resource="http://www.w3.org/2001/XMLSchema#string"/>
  </owl:DatatypeProperty>
  <owl:DatatypeProperty rdf:about="http://example.org/onto/prop/google_compute_region_url_map_allow_methods">
    <rdfs:label>allow_methods</rdfs:label>
    <rdfs:comment>Specifies the content for the Access-Control-Allow-Methods header.</rdfs:comment>
    <rdfs:domain rdf:resource="http://example.org/onto/class/google_compute_region_url_map"/>
    <rdfs:range rdf:resource="http://www.w3.org/2001/XMLSchema#string"/>
  </owl:DatatypeProperty>
  <owl:DatatypeProperty rdf:about="http://example.org/onto/prop/google_compute_region_url_map_allow_origin_regexes">
    <rdfs:label>allow_origin_regexes</rdfs:label>
    <rdfs:comment>Specifies the regular expression patterns that match allowed origins. For
regular expression grammar please see en.cppreference.com/w/cpp/regex/ecmascript
An origin is allowed if it matches either allow_origins or allow_origin_regex.</rdfs:comment>
    <rdfs:domain rdf:resource="http://example.org/onto/class/google_compute_region_url_map"/>
    <rdfs:range rdf:resource="http://www.w3.org/2001/XMLSchema#string"/>
  </owl:DatatypeProperty>
  <owl:DatatypeProperty rdf:about="http://example.org/onto/prop/google_compute_region_url_map_allow_origins">
    <rdfs:label>allow_origins</rdfs:label>
    <rdfs:comment>Specifies the list of origins that will be allowed to do CORS requests. An
origin is allowed if it matches either allow_origins or allow_origin_regex.</rdfs:comment>
    <rdfs:domain rdf:resource="http://example.org/onto/class/google_compute_region_url_map"/>
    <rdfs:range rdf:resource="http://www.w3.org/2001/XMLSchema#string"/>
  </owl:DatatypeProperty>
  <owl:DatatypeProperty rdf:about="http://example.org/onto/prop/google_compute_region_url_map_disabled">
    <rdfs:label>disabled</rdfs:label>
    <rdfs:comment>If true, specifies the CORS policy is disabled.</rdfs:comment>
    <rdfs:domain rdf:resource="http://example.org/onto/class/google_compute_region_url_map"/>
    <rdfs:range rdf:resource="http://www.w3.org/2001/XMLSchema#string"/>
  </owl:DatatypeProperty>
  <owl:DatatypeProperty rdf:about="http://example.org/onto/prop/google_compute_region_url_map_expose_headers">
    <rdfs:label>expose_headers</rdfs:label>
    <rdfs:comment>Specifies the content for the Access-Control-Expose-Headers header.</rdfs:comment>
    <rdfs:domain rdf:resource="http://example.org/onto/class/google_compute_region_url_map"/>
    <rdfs:range rdf:resource="http://www.w3.org/2001/XMLSchema#string"/>
  </owl:DatatypeProperty>
  <owl:DatatypeProperty rdf:about="http://example.org/onto/prop/google_compute_region_url_map_max_age">
    <rdfs:label>max_age</rdfs:label>
    <rdfs:comment>Specifies how long the results of a preflight request can be cached. This
translates to the content for the Access-Control-Max-Age header.</rdfs:comment>
    <rdfs:domain rdf:resource="http://example.org/onto/class/google_compute_region_url_map"/>
    <rdfs:range rdf:resource="http://www.w3.org/2001/XMLSchema#string"/>
  </owl:DatatypeProperty>
  <owl:DatatypeProperty rdf:about="http://example.org/onto/prop/google_compute_region_url_map_http_status">
    <rdfs:label>http_status</rdfs:label>
    <rdfs:comment>The HTTP status code used to abort the request. The value must be between 200
and 599 inclusive.</rdfs:comment>
    <rdfs:domain rdf:resource="http://example.org/onto/class/google_compute_region_url_map"/>
    <rdfs:range rdf:resource="http://www.w3.org/2001/XMLSchema#string"/>
  </owl:DatatypeProperty>
  <owl:DatatypeProperty rdf:about="http://example.org/onto/prop/google_compute_region_url_map_percentage">
    <rdfs:label>percentage</rdfs:label>
    <rdfs:comment>The percentage of traffic (connections/operations/requests) which will be
aborted as part of fault injection. The value must be between 0.0 and 100.0
inclusive.</rdfs:comment>
    <rdfs:domain rdf:resource="http://example.org/onto/class/google_compute_region_url_map"/>
    <rdfs:range rdf:resource="http://www.w3.org/2001/XMLSchema#string"/>
  </owl:DatatypeProperty>
  <owl:DatatypeProperty rdf:about="http://example.org/onto/prop/google_compute_region_url_map_percentage">
    <rdfs:label>percentage</rdfs:label>
    <rdfs:comment>The percentage of traffic (connections/operations/requests) on which delay will
be introduced as part of fault injection. The value must be between 0.0 and
100.0 inclusive.</rdfs:comment>
    <rdfs:domain rdf:resource="http://example.org/onto/class/google_compute_region_url_map"/>
    <rdfs:range rdf:resource="http://www.w3.org/2001/XMLSchema#string"/>
  </owl:DatatypeProperty>
  <owl:DatatypeProperty rdf:about="http://example.org/onto/prop/google_compute_region_url_map_nanos">
    <rdfs:label>nanos</rdfs:label>
    <rdfs:comment>Span of time that's a fraction of a second at nanosecond resolution. Durations
less than one second are represented with a 0 'seconds' field and a positive
'nanos' field. Must be from 0 to 999,999,999 inclusive.</rdfs:comment>
    <rdfs:domain rdf:resource="http://example.org/onto/class/google_compute_region_url_map"/>
    <rdfs:range rdf:resource="http://www.w3.org/2001/XMLSchema#string"/>
  </owl:DatatypeProperty>
  <owl:DatatypeProperty rdf:about="http://example.org/onto/prop/google_compute_region_url_map_seconds">
    <rdfs:label>seconds</rdfs:label>
    <rdfs:comment>Span of time at a resolution of a second. Must be from 0 to 315,576,000,000
inclusive.</rdfs:comment>
    <rdfs:domain rdf:resource="http://example.org/onto/class/google_compute_region_url_map"/>
    <rdfs:range rdf:resource="http://www.w3.org/2001/XMLSchema#string"/>
  </owl:DatatypeProperty>
  <owl:DatatypeProperty rdf:about="http://example.org/onto/prop/google_compute_region_url_map_backend_service">
    <rdfs:label>backend_service</rdfs:label>
    <rdfs:comment>The RegionBackendService resource being mirrored to.</rdfs:comment>
    <rdfs:domain rdf:resource="http://example.org/onto/class/google_compute_region_url_map"/>
    <rdfs:range rdf:resource="http://www.w3.org/2001/XMLSchema#string"/>
  </owl:DatatypeProperty>
  <owl:DatatypeProperty rdf:about="http://example.org/onto/prop/google_compute_region_url_map_num_retries">
    <rdfs:label>num_retries</rdfs:label>
    <rdfs:comment>Specifies the allowed number retries. This number must be > 0.</rdfs:comment>
    <rdfs:domain rdf:resource="http://example.org/onto/class/google_compute_region_url_map"/>
    <rdfs:range rdf:resource="http://www.w3.org/2001/XMLSchema#string"/>
  </owl:DatatypeProperty>
  <owl:DatatypeProperty rdf:about="http://example.org/onto/prop/google_compute_region_url_map_retry_conditions">
    <rdfs:label>retry_conditions</rdfs:label>
    <rdfs:comment>Specifies one or more conditions when this retry rule applies. Valid values are:

- 5xx: Loadbalancer will attempt a retry if the backend service responds with
any 5xx response code, or if the backend service does not respond at all,
for example: disconnects, reset, read timeout, connection failure, and refused
streams.
- gateway-error: Similar to 5xx, but only applies to response codes
502, 503 or 504.
- connect-failure: Loadbalancer will retry on failures
connecting to backend services, for example due to connection timeouts.
- retriable-4xx: Loadbalancer will retry for retriable 4xx response codes.
Currently the only retriable error supported is 409.
- refused-stream: Loadbalancer will retry if the backend service resets the stream with a
REFUSED_STREAM error code. This reset type indicates that it is safe to retry.
- cancelled: Loadbalancer will retry if the gRPC status code in the response
header is set to cancelled
- deadline-exceeded: Loadbalancer will retry if the
gRPC status code in the response header is set to deadline-exceeded
- resource-exhausted: Loadbalancer will retry if the gRPC status code in the response
header is set to resource-exhausted
- unavailable: Loadbalancer will retry if
the gRPC status code in the response header is set to unavailable</rdfs:comment>
    <rdfs:domain rdf:resource="http://example.org/onto/class/google_compute_region_url_map"/>
    <rdfs:range rdf:resource="http://www.w3.org/2001/XMLSchema#string"/>
  </owl:DatatypeProperty>
  <owl:DatatypeProperty rdf:about="http://example.org/onto/prop/google_compute_region_url_map_nanos">
    <rdfs:label>nanos</rdfs:label>
    <rdfs:comment>Span of time that's a fraction of a second at nanosecond resolution. Durations
less than one second are represented with a 0 'seconds' field and a positive
'nanos' field. Must be from 0 to 999,999,999 inclusive.</rdfs:comment>
    <rdfs:domain rdf:resource="http://example.org/onto/class/google_compute_region_url_map"/>
    <rdfs:range rdf:resource="http://www.w3.org/2001/XMLSchema#string"/>
  </owl:DatatypeProperty>
  <owl:DatatypeProperty rdf:about="http://example.org/onto/prop/google_compute_region_url_map_seconds">
    <rdfs:label>seconds</rdfs:label>
    <rdfs:comment>Span of time at a resolution of a second. Must be from 0 to 315,576,000,000
inclusive.</rdfs:comment>
    <rdfs:domain rdf:resource="http://example.org/onto/class/google_compute_region_url_map"/>
    <rdfs:range rdf:resource="http://www.w3.org/2001/XMLSchema#string"/>
  </owl:DatatypeProperty>
  <owl:DatatypeProperty rdf:about="http://example.org/onto/prop/google_compute_region_url_map_nanos">
    <rdfs:label>nanos</rdfs:label>
    <rdfs:comment>Span of time that's a fraction of a second at nanosecond resolution. Durations
less than one second are represented with a 0 'seconds' field and a positive
'nanos' field. Must be from 0 to 999,999,999 inclusive.</rdfs:comment>
    <rdfs:domain rdf:resource="http://example.org/onto/class/google_compute_region_url_map"/>
    <rdfs:range rdf:resource="http://www.w3.org/2001/XMLSchema#string"/>
  </owl:DatatypeProperty>
  <owl:DatatypeProperty rdf:about="http://example.org/onto/prop/google_compute_region_url_map_seconds">
    <rdfs:label>seconds</rdfs:label>
    <rdfs:comment>Span of time at a resolution of a second. Must be from 0 to 315,576,000,000
inclusive.</rdfs:comment>
    <rdfs:domain rdf:resource="http://example.org/onto/class/google_compute_region_url_map"/>
    <rdfs:range rdf:resource="http://www.w3.org/2001/XMLSchema#string"/>
  </owl:DatatypeProperty>
  <owl:DatatypeProperty rdf:about="http://example.org/onto/prop/google_compute_region_url_map_host_rewrite">
    <rdfs:label>host_rewrite</rdfs:label>
    <rdfs:comment>Prior to forwarding the request to the selected service, the request's host
header is replaced with contents of hostRewrite. The value must be between 1 and
255 characters.</rdfs:comment>
    <rdfs:domain rdf:resource="http://example.org/onto/class/google_compute_region_url_map"/>
    <rdfs:range rdf:resource="http://www.w3.org/2001/XMLSchema#string"/>
  </owl:DatatypeProperty>
  <owl:DatatypeProperty rdf:about="http://example.org/onto/prop/google_compute_region_url_map_path_prefix_rewrite">
    <rdfs:label>path_prefix_rewrite</rdfs:label>
    <rdfs:comment>Prior to forwarding the request to the selected backend service, the matching
portion of the request's path is replaced by pathPrefixRewrite. The value must
be between 1 and 1024 characters.</rdfs:comment>
    <rdfs:domain rdf:resource="http://example.org/onto/class/google_compute_region_url_map"/>
    <rdfs:range rdf:resource="http://www.w3.org/2001/XMLSchema#string"/>
  </owl:DatatypeProperty>
  <owl:DatatypeProperty rdf:about="http://example.org/onto/prop/google_compute_region_url_map_backend_service">
    <rdfs:label>backend_service</rdfs:label>
    <rdfs:comment>The default RegionBackendService resource. Before
forwarding the request to backendService, the loadbalancer applies any relevant
headerActions specified as part of this backendServiceWeight.</rdfs:comment>
    <rdfs:domain rdf:resource="http://example.org/onto/class/google_compute_region_url_map"/>
    <rdfs:range rdf:resource="http://www.w3.org/2001/XMLSchema#string"/>
  </owl:DatatypeProperty>
  <owl:DatatypeProperty rdf:about="http://example.org/onto/prop/google_compute_region_url_map_weight">
    <rdfs:label>weight</rdfs:label>
    <rdfs:comment>Specifies the fraction of traffic sent to backendService, computed as weight /
(sum of all weightedBackendService weights in routeAction) . The selection of a
backend service is determined only for new traffic. Once a user's request has
been directed to a backendService, subsequent requests will be sent to the same
backendService as determined by the BackendService's session affinity policy.
The value must be between 0 and 1000</rdfs:comment>
    <rdfs:domain rdf:resource="http://example.org/onto/class/google_compute_region_url_map"/>
    <rdfs:range rdf:resource="http://www.w3.org/2001/XMLSchema#string"/>
  </owl:DatatypeProperty>
  <owl:DatatypeProperty rdf:about="http://example.org/onto/prop/google_compute_region_url_map_request_headers_to_remove">
    <rdfs:label>request_headers_to_remove</rdfs:label>
    <rdfs:comment>A list of header names for headers that need to be removed from the request
prior to forwarding the request to the backendService.</rdfs:comment>
    <rdfs:domain rdf:resource="http://example.org/onto/class/google_compute_region_url_map"/>
    <rdfs:range rdf:resource="http://www.w3.org/2001/XMLSchema#string"/>
  </owl:DatatypeProperty>
  <owl:DatatypeProperty rdf:about="http://example.org/onto/prop/google_compute_region_url_map_response_headers_to_remove">
    <rdfs:label>response_headers_to_remove</rdfs:label>
    <rdfs:comment>A list of header names for headers that need to be removed from the response
prior to sending the response back to the client.</rdfs:comment>
    <rdfs:domain rdf:resource="http://example.org/onto/class/google_compute_region_url_map"/>
    <rdfs:range rdf:resource="http://www.w3.org/2001/XMLSchema#string"/>
  </owl:DatatypeProperty>
  <owl:DatatypeProperty rdf:about="http://example.org/onto/prop/google_compute_region_url_map_header_name">
    <rdfs:label>header_name</rdfs:label>
    <rdfs:comment>The name of the header.</rdfs:comment>
    <rdfs:domain rdf:resource="http://example.org/onto/class/google_compute_region_url_map"/>
    <rdfs:range rdf:resource="http://www.w3.org/2001/XMLSchema#string"/>
  </owl:DatatypeProperty>
  <owl:DatatypeProperty rdf:about="http://example.org/onto/prop/google_compute_region_url_map_header_value">
    <rdfs:label>header_value</rdfs:label>
    <rdfs:comment>The value of the header to add.</rdfs:comment>
    <rdfs:domain rdf:resource="http://example.org/onto/class/google_compute_region_url_map"/>
    <rdfs:range rdf:resource="http://www.w3.org/2001/XMLSchema#string"/>
  </owl:DatatypeProperty>
  <owl:DatatypeProperty rdf:about="http://example.org/onto/prop/google_compute_region_url_map_replace">
    <rdfs:label>replace</rdfs:label>
    <rdfs:comment>If false, headerValue is appended to any values that already exist for the
header. If true, headerValue is set for the header, discarding any values that
were set for that header.</rdfs:comment>
    <rdfs:domain rdf:resource="http://example.org/onto/class/google_compute_region_url_map"/>
    <rdfs:range rdf:resource="http://www.w3.org/2001/XMLSchema#string"/>
  </owl:DatatypeProperty>
  <owl:DatatypeProperty rdf:about="http://example.org/onto/prop/google_compute_region_url_map_header_name">
    <rdfs:label>header_name</rdfs:label>
    <rdfs:comment>The name of the header.</rdfs:comment>
    <rdfs:domain rdf:resource="http://example.org/onto/class/google_compute_region_url_map"/>
    <rdfs:range rdf:resource="http://www.w3.org/2001/XMLSchema#string"/>
  </owl:DatatypeProperty>
  <owl:DatatypeProperty rdf:about="http://example.org/onto/prop/google_compute_region_url_map_header_value">
    <rdfs:label>header_value</rdfs:label>
    <rdfs:comment>The value of the header to add.</rdfs:comment>
    <rdfs:domain rdf:resource="http://example.org/onto/class/google_compute_region_url_map"/>
    <rdfs:range rdf:resource="http://www.w3.org/2001/XMLSchema#string"/>
  </owl:DatatypeProperty>
  <owl:DatatypeProperty rdf:about="http://example.org/onto/prop/google_compute_region_url_map_replace">
    <rdfs:label>replace</rdfs:label>
    <rdfs:comment>If false, headerValue is appended to any values that already exist for the
header. If true, headerValue is set for the header, discarding any values that
were set for that header.</rdfs:comment>
    <rdfs:domain rdf:resource="http://example.org/onto/class/google_compute_region_url_map"/>
    <rdfs:range rdf:resource="http://www.w3.org/2001/XMLSchema#string"/>
  </owl:DatatypeProperty>
  <owl:DatatypeProperty rdf:about="http://example.org/onto/prop/google_compute_region_url_map_host_redirect">
    <rdfs:label>host_redirect</rdfs:label>
    <rdfs:comment>The host that will be used in the redirect response instead of the one
that was supplied in the request. The value must be between 1 and 255
characters.</rdfs:comment>
    <rdfs:domain rdf:resource="http://example.org/onto/class/google_compute_region_url_map"/>
    <rdfs:range rdf:resource="http://www.w3.org/2001/XMLSchema#string"/>
  </owl:DatatypeProperty>
  <owl:DatatypeProperty rdf:about="http://example.org/onto/prop/google_compute_region_url_map_https_redirect">
    <rdfs:label>https_redirect</rdfs:label>
    <rdfs:comment>If set to true, the URL scheme in the redirected request is set to https.
If set to false, the URL scheme of the redirected request will remain the
same as that of the request. This must only be set for UrlMaps used in
TargetHttpProxys. Setting this true for TargetHttpsProxy is not
permitted. The default is set to false.</rdfs:comment>
    <rdfs:domain rdf:resource="http://example.org/onto/class/google_compute_region_url_map"/>
    <rdfs:range rdf:resource="http://www.w3.org/2001/XMLSchema#string"/>
  </owl:DatatypeProperty>
  <owl:DatatypeProperty rdf:about="http://example.org/onto/prop/google_compute_region_url_map_path_redirect">
    <rdfs:label>path_redirect</rdfs:label>
    <rdfs:comment>The path that will be used in the redirect response instead of the one
that was supplied in the request. pathRedirect cannot be supplied
together with prefixRedirect. Supply one alone or neither. If neither is
supplied, the path of the original request will be used for the redirect.
The value must be between 1 and 1024 characters.</rdfs:comment>
    <rdfs:domain rdf:resource="http://example.org/onto/class/google_compute_region_url_map"/>
    <rdfs:range rdf:resource="http://www.w3.org/2001/XMLSchema#string"/>
  </owl:DatatypeProperty>
  <owl:DatatypeProperty rdf:about="http://example.org/onto/prop/google_compute_region_url_map_prefix_redirect">
    <rdfs:label>prefix_redirect</rdfs:label>
    <rdfs:comment>The prefix that replaces the prefixMatch specified in the
HttpRouteRuleMatch, retaining the remaining portion of the URL before
redirecting the request. prefixRedirect cannot be supplied together with
pathRedirect. Supply one alone or neither. If neither is supplied, the
path of the original request will be used for the redirect. The value
must be between 1 and 1024 characters.</rdfs:comment>
    <rdfs:domain rdf:resource="http://example.org/onto/class/google_compute_region_url_map"/>
    <rdfs:range rdf:resource="http://www.w3.org/2001/XMLSchema#string"/>
  </owl:DatatypeProperty>
  <owl:DatatypeProperty rdf:about="http://example.org/onto/prop/google_compute_region_url_map_redirect_response_code">
    <rdfs:label>redirect_response_code</rdfs:label>
    <rdfs:comment>The HTTP Status code to use for this RedirectAction. Supported values are:

* MOVED_PERMANENTLY_DEFAULT, which is the default value and corresponds to 301.

* FOUND, which corresponds to 302.

* SEE_OTHER which corresponds to 303.

* TEMPORARY_REDIRECT, which corresponds to 307. In this case, the request method
will be retained.

* PERMANENT_REDIRECT, which corresponds to 308. In this case,
the request method will be retained. Possible values: ["FOUND", "MOVED_PERMANENTLY_DEFAULT", "PERMANENT_REDIRECT", "SEE_OTHER", "TEMPORARY_REDIRECT"]</rdfs:comment>
    <rdfs:domain rdf:resource="http://example.org/onto/class/google_compute_region_url_map"/>
    <rdfs:range rdf:resource="http://www.w3.org/2001/XMLSchema#string"/>
  </owl:DatatypeProperty>
  <owl:DatatypeProperty rdf:about="http://example.org/onto/prop/google_compute_region_url_map_strip_query">
    <rdfs:label>strip_query</rdfs:label>
    <rdfs:comment>If set to true, any accompanying query portion of the original URL is removed
prior to redirecting the request. If set to false, the query portion of the
original URL is retained.
 This field is required to ensure an empty block is not set. The normal default value is false.</rdfs:comment>
    <rdfs:domain rdf:resource="http://example.org/onto/class/google_compute_region_url_map"/>
    <rdfs:range rdf:resource="http://www.w3.org/2001/XMLSchema#string"/>
  </owl:DatatypeProperty>
  <owl:DatatypeProperty rdf:about="http://example.org/onto/prop/google_compute_region_url_map_priority">
    <rdfs:label>priority</rdfs:label>
    <rdfs:comment>For routeRules within a given pathMatcher, priority determines the order
in which load balancer will interpret routeRules. RouteRules are evaluated
in order of priority, from the lowest to highest number. The priority of
a rule decreases as its number increases (1, 2, 3, N+1). The first rule
that matches the request is applied.

You cannot configure two or more routeRules with the same priority.
Priority for each rule must be set to a number between 0 and
2147483647 inclusive.

Priority numbers can have gaps, which enable you to add or remove rules
in the future without affecting the rest of the rules. For example,
1, 2, 3, 4, 5, 9, 12, 16 is a valid series of priority numbers to which
you could add rules numbered from 6 to 8, 10 to 11, and 13 to 15 in the
future without any impact on existing rules.</rdfs:comment>
    <rdfs:domain rdf:resource="http://example.org/onto/class/google_compute_region_url_map"/>
    <rdfs:range rdf:resource="http://www.w3.org/2001/XMLSchema#string"/>
  </owl:DatatypeProperty>
  <owl:DatatypeProperty rdf:about="http://example.org/onto/prop/google_compute_region_url_map_service">
    <rdfs:label>service</rdfs:label>
    <rdfs:comment>The region backend service resource to which traffic is
directed if this rule is matched. If routeAction is additionally specified,
advanced routing actions like URL Rewrites, etc. take effect prior to sending
the request to the backend. However, if service is specified, routeAction cannot
contain any weightedBackendService s. Conversely, if routeAction specifies any
weightedBackendServices, service must not be specified. Only one of urlRedirect,
service or routeAction.weightedBackendService must be set.</rdfs:comment>
    <rdfs:domain rdf:resource="http://example.org/onto/class/google_compute_region_url_map"/>
    <rdfs:range rdf:resource="http://www.w3.org/2001/XMLSchema#string"/>
  </owl:DatatypeProperty>
  <owl:DatatypeProperty rdf:about="http://example.org/onto/prop/google_compute_region_url_map_request_headers_to_remove">
    <rdfs:label>request_headers_to_remove</rdfs:label>
    <rdfs:comment>A list of header names for headers that need to be removed from the request
prior to forwarding the request to the backendService.</rdfs:comment>
    <rdfs:domain rdf:resource="http://example.org/onto/class/google_compute_region_url_map"/>
    <rdfs:range rdf:resource="http://www.w3.org/2001/XMLSchema#string"/>
  </owl:DatatypeProperty>
  <owl:DatatypeProperty rdf:about="http://example.org/onto/prop/google_compute_region_url_map_response_headers_to_remove">
    <rdfs:label>response_headers_to_remove</rdfs:label>
    <rdfs:comment>A list of header names for headers that need to be removed from the response
prior to sending the response back to the client.</rdfs:comment>
    <rdfs:domain rdf:resource="http://example.org/onto/class/google_compute_region_url_map"/>
    <rdfs:range rdf:resource="http://www.w3.org/2001/XMLSchema#string"/>
  </owl:DatatypeProperty>
  <owl:DatatypeProperty rdf:about="http://example.org/onto/prop/google_compute_region_url_map_header_name">
    <rdfs:label>header_name</rdfs:label>
    <rdfs:comment>The name of the header.</rdfs:comment>
    <rdfs:domain rdf:resource="http://example.org/onto/class/google_compute_region_url_map"/>
    <rdfs:range rdf:resource="http://www.w3.org/2001/XMLSchema#string"/>
  </owl:DatatypeProperty>
  <owl:DatatypeProperty rdf:about="http://example.org/onto/prop/google_compute_region_url_map_header_value">
    <rdfs:label>header_value</rdfs:label>
    <rdfs:comment>The value of the header to add.</rdfs:comment>
    <rdfs:domain rdf:resource="http://example.org/onto/class/google_compute_region_url_map"/>
    <rdfs:range rdf:resource="http://www.w3.org/2001/XMLSchema#string"/>
  </owl:DatatypeProperty>
  <owl:DatatypeProperty rdf:about="http://example.org/onto/prop/google_compute_region_url_map_replace">
    <rdfs:label>replace</rdfs:label>
    <rdfs:comment>If false, headerValue is appended to any values that already exist for the
header. If true, headerValue is set for the header, discarding any values that
were set for that header.</rdfs:comment>
    <rdfs:domain rdf:resource="http://example.org/onto/class/google_compute_region_url_map"/>
    <rdfs:range rdf:resource="http://www.w3.org/2001/XMLSchema#string"/>
  </owl:DatatypeProperty>
  <owl:DatatypeProperty rdf:about="http://example.org/onto/prop/google_compute_region_url_map_header_name">
    <rdfs:label>header_name</rdfs:label>
    <rdfs:comment>The name of the header.</rdfs:comment>
    <rdfs:domain rdf:resource="http://example.org/onto/class/google_compute_region_url_map"/>
    <rdfs:range rdf:resource="http://www.w3.org/2001/XMLSchema#string"/>
  </owl:DatatypeProperty>
  <owl:DatatypeProperty rdf:about="http://example.org/onto/prop/google_compute_region_url_map_header_value">
    <rdfs:label>header_value</rdfs:label>
    <rdfs:comment>The value of the header to add.</rdfs:comment>
    <rdfs:domain rdf:resource="http://example.org/onto/class/google_compute_region_url_map"/>
    <rdfs:range rdf:resource="http://www.w3.org/2001/XMLSchema#string"/>
  </owl:DatatypeProperty>
  <owl:DatatypeProperty rdf:about="http://example.org/onto/prop/google_compute_region_url_map_replace">
    <rdfs:label>replace</rdfs:label>
    <rdfs:comment>If false, headerValue is appended to any values that already exist for the
header. If true, headerValue is set for the header, discarding any values that
were set for that header.</rdfs:comment>
    <rdfs:domain rdf:resource="http://example.org/onto/class/google_compute_region_url_map"/>
    <rdfs:range rdf:resource="http://www.w3.org/2001/XMLSchema#string"/>
  </owl:DatatypeProperty>
  <owl:DatatypeProperty rdf:about="http://example.org/onto/prop/google_compute_region_url_map_full_path_match">
    <rdfs:label>full_path_match</rdfs:label>
    <rdfs:comment>For satisfying the matchRule condition, the path of the request must exactly
match the value specified in fullPathMatch after removing any query parameters
and anchor that may be part of the original URL. FullPathMatch must be between 1
and 1024 characters. Only one of prefixMatch, fullPathMatch or regexMatch must
be specified.</rdfs:comment>
    <rdfs:domain rdf:resource="http://example.org/onto/class/google_compute_region_url_map"/>
    <rdfs:range rdf:resource="http://www.w3.org/2001/XMLSchema#string"/>
  </owl:DatatypeProperty>
  <owl:DatatypeProperty rdf:about="http://example.org/onto/prop/google_compute_region_url_map_ignore_case">
    <rdfs:label>ignore_case</rdfs:label>
    <rdfs:comment>Specifies that prefixMatch and fullPathMatch matches are case sensitive.
Defaults to false.</rdfs:comment>
    <rdfs:domain rdf:resource="http://example.org/onto/class/google_compute_region_url_map"/>
    <rdfs:range rdf:resource="http://www.w3.org/2001/XMLSchema#string"/>
  </owl:DatatypeProperty>
  <owl:DatatypeProperty rdf:about="http://example.org/onto/prop/google_compute_region_url_map_path_template_match">
    <rdfs:label>path_template_match</rdfs:label>
    <rdfs:comment>For satisfying the matchRule condition, the path of the request
must match the wildcard pattern specified in pathTemplateMatch
after removing any query parameters and anchor that may be part
of the original URL.

pathTemplateMatch must be between 1 and 255 characters
(inclusive).  The pattern specified by pathTemplateMatch may
have at most 5 wildcard operators and at most 5 variable
captures in total.</rdfs:comment>
    <rdfs:domain rdf:resource="http://example.org/onto/class/google_compute_region_url_map"/>
    <rdfs:range rdf:resource="http://www.w3.org/2001/XMLSchema#string"/>
  </owl:DatatypeProperty>
  <owl:DatatypeProperty rdf:about="http://example.org/onto/prop/google_compute_region_url_map_prefix_match">
    <rdfs:label>prefix_match</rdfs:label>
    <rdfs:comment>For satisfying the matchRule condition, the request's path must begin with the
specified prefixMatch. prefixMatch must begin with a /. The value must be
between 1 and 1024 characters. Only one of prefixMatch, fullPathMatch or
regexMatch must be specified.</rdfs:comment>
    <rdfs:domain rdf:resource="http://example.org/onto/class/google_compute_region_url_map"/>
    <rdfs:range rdf:resource="http://www.w3.org/2001/XMLSchema#string"/>
  </owl:DatatypeProperty>
  <owl:DatatypeProperty rdf:about="http://example.org/onto/prop/google_compute_region_url_map_regex_match">
    <rdfs:label>regex_match</rdfs:label>
    <rdfs:comment>For satisfying the matchRule condition, the path of the request must satisfy the
regular expression specified in regexMatch after removing any query parameters
and anchor supplied with the original URL. For regular expression grammar please
see en.cppreference.com/w/cpp/regex/ecmascript  Only one of prefixMatch,
fullPathMatch or regexMatch must be specified.</rdfs:comment>
    <rdfs:domain rdf:resource="http://example.org/onto/class/google_compute_region_url_map"/>
    <rdfs:range rdf:resource="http://www.w3.org/2001/XMLSchema#string"/>
  </owl:DatatypeProperty>
  <owl:DatatypeProperty rdf:about="http://example.org/onto/prop/google_compute_region_url_map_exact_match">
    <rdfs:label>exact_match</rdfs:label>
    <rdfs:comment>The value should exactly match contents of exactMatch. Only one of exactMatch,
prefixMatch, suffixMatch, regexMatch, presentMatch or rangeMatch must be set.</rdfs:comment>
    <rdfs:domain rdf:resource="http://example.org/onto/class/google_compute_region_url_map"/>
    <rdfs:range rdf:resource="http://www.w3.org/2001/XMLSchema#string"/>
  </owl:DatatypeProperty>
  <owl:DatatypeProperty rdf:about="http://example.org/onto/prop/google_compute_region_url_map_header_name">
    <rdfs:label>header_name</rdfs:label>
    <rdfs:comment>The name of the HTTP header to match. For matching against the HTTP request's
authority, use a headerMatch with the header name ":authority". For matching a
request's method, use the headerName ":method".</rdfs:comment>
    <rdfs:domain rdf:resource="http://example.org/onto/class/google_compute_region_url_map"/>
    <rdfs:range rdf:resource="http://www.w3.org/2001/XMLSchema#string"/>
  </owl:DatatypeProperty>
  <owl:DatatypeProperty rdf:about="http://example.org/onto/prop/google_compute_region_url_map_invert_match">
    <rdfs:label>invert_match</rdfs:label>
    <rdfs:comment>If set to false, the headerMatch is considered a match if the match criteria
above are met. If set to true, the headerMatch is considered a match if the
match criteria above are NOT met. Defaults to false.</rdfs:comment>
    <rdfs:domain rdf:resource="http://example.org/onto/class/google_compute_region_url_map"/>
    <rdfs:range rdf:resource="http://www.w3.org/2001/XMLSchema#string"/>
  </owl:DatatypeProperty>
  <owl:DatatypeProperty rdf:about="http://example.org/onto/prop/google_compute_region_url_map_prefix_match">
    <rdfs:label>prefix_match</rdfs:label>
    <rdfs:comment>The value of the header must start with the contents of prefixMatch. Only one of
exactMatch, prefixMatch, suffixMatch, regexMatch, presentMatch or rangeMatch
must be set.</rdfs:comment>
    <rdfs:domain rdf:resource="http://example.org/onto/class/google_compute_region_url_map"/>
    <rdfs:range rdf:resource="http://www.w3.org/2001/XMLSchema#string"/>
  </owl:DatatypeProperty>
  <owl:DatatypeProperty rdf:about="http://example.org/onto/prop/google_compute_region_url_map_present_match">
    <rdfs:label>present_match</rdfs:label>
    <rdfs:comment>A header with the contents of headerName must exist. The match takes place
whether or not the request's header has a value or not. Only one of exactMatch,
prefixMatch, suffixMatch, regexMatch, presentMatch or rangeMatch must be set.</rdfs:comment>
    <rdfs:domain rdf:resource="http://example.org/onto/class/google_compute_region_url_map"/>
    <rdfs:range rdf:resource="http://www.w3.org/2001/XMLSchema#string"/>
  </owl:DatatypeProperty>
  <owl:DatatypeProperty rdf:about="http://example.org/onto/prop/google_compute_region_url_map_regex_match">
    <rdfs:label>regex_match</rdfs:label>
    <rdfs:comment>The value of the header must match the regular expression specified in
regexMatch. For regular expression grammar, please see:
en.cppreference.com/w/cpp/regex/ecmascript  For matching against a port
specified in the HTTP request, use a headerMatch with headerName set to PORT and
a regular expression that satisfies the RFC2616 Host header's port specifier.
Only one of exactMatch, prefixMatch, suffixMatch, regexMatch, presentMatch or
rangeMatch must be set.</rdfs:comment>
    <rdfs:domain rdf:resource="http://example.org/onto/class/google_compute_region_url_map"/>
    <rdfs:range rdf:resource="http://www.w3.org/2001/XMLSchema#string"/>
  </owl:DatatypeProperty>
  <owl:DatatypeProperty rdf:about="http://example.org/onto/prop/google_compute_region_url_map_suffix_match">
    <rdfs:label>suffix_match</rdfs:label>
    <rdfs:comment>The value of the header must end with the contents of suffixMatch. Only one of
exactMatch, prefixMatch, suffixMatch, regexMatch, presentMatch or rangeMatch
must be set.</rdfs:comment>
    <rdfs:domain rdf:resource="http://example.org/onto/class/google_compute_region_url_map"/>
    <rdfs:range rdf:resource="http://www.w3.org/2001/XMLSchema#string"/>
  </owl:DatatypeProperty>
  <owl:DatatypeProperty rdf:about="http://example.org/onto/prop/google_compute_region_url_map_range_end">
    <rdfs:label>range_end</rdfs:label>
    <rdfs:comment>The end of the range (exclusive).</rdfs:comment>
    <rdfs:domain rdf:resource="http://example.org/onto/class/google_compute_region_url_map"/>
    <rdfs:range rdf:resource="http://www.w3.org/2001/XMLSchema#string"/>
  </owl:DatatypeProperty>
  <owl:DatatypeProperty rdf:about="http://example.org/onto/prop/google_compute_region_url_map_range_start">
    <rdfs:label>range_start</rdfs:label>
    <rdfs:comment>The start of the range (inclusive).</rdfs:comment>
    <rdfs:domain rdf:resource="http://example.org/onto/class/google_compute_region_url_map"/>
    <rdfs:range rdf:resource="http://www.w3.org/2001/XMLSchema#string"/>
  </owl:DatatypeProperty>
  <owl:DatatypeProperty rdf:about="http://example.org/onto/prop/google_compute_region_url_map_filter_match_criteria">
    <rdfs:label>filter_match_criteria</rdfs:label>
    <rdfs:comment>Specifies how individual filterLabel matches within the list of filterLabels
contribute towards the overall metadataFilter match. Supported values are:

* MATCH_ANY: At least one of the filterLabels must have a matching label in the
provided metadata.
* MATCH_ALL: All filterLabels must have matching labels in
the provided metadata. Possible values: ["MATCH_ALL", "MATCH_ANY"]</rdfs:comment>
    <rdfs:domain rdf:resource="http://example.org/onto/class/google_compute_region_url_map"/>
    <rdfs:range rdf:resource="http://www.w3.org/2001/XMLSchema#string"/>
  </owl:DatatypeProperty>
  <owl:DatatypeProperty rdf:about="http://example.org/onto/prop/google_compute_region_url_map_name">
    <rdfs:label>name</rdfs:label>
    <rdfs:comment>Name of metadata label. The name can have a maximum length of 1024 characters
and must be at least 1 character long.</rdfs:comment>
    <rdfs:domain rdf:resource="http://example.org/onto/class/google_compute_region_url_map"/>
    <rdfs:range rdf:resource="http://www.w3.org/2001/XMLSchema#string"/>
  </owl:DatatypeProperty>
  <owl:DatatypeProperty rdf:about="http://example.org/onto/prop/google_compute_region_url_map_value">
    <rdfs:label>value</rdfs:label>
    <rdfs:comment>The value of the label must match the specified value. value can have a maximum
length of 1024 characters.</rdfs:comment>
    <rdfs:domain rdf:resource="http://example.org/onto/class/google_compute_region_url_map"/>
    <rdfs:range rdf:resource="http://www.w3.org/2001/XMLSchema#string"/>
  </owl:DatatypeProperty>
  <owl:DatatypeProperty rdf:about="http://example.org/onto/prop/google_compute_region_url_map_exact_match">
    <rdfs:label>exact_match</rdfs:label>
    <rdfs:comment>The queryParameterMatch matches if the value of the parameter exactly matches
the contents of exactMatch. Only one of presentMatch, exactMatch and regexMatch
must be set.</rdfs:comment>
    <rdfs:domain rdf:resource="http://example.org/onto/class/google_compute_region_url_map"/>
    <rdfs:range rdf:resource="http://www.w3.org/2001/XMLSchema#string"/>
  </owl:DatatypeProperty>
  <owl:DatatypeProperty rdf:about="http://example.org/onto/prop/google_compute_region_url_map_name">
    <rdfs:label>name</rdfs:label>
    <rdfs:comment>The name of the query parameter to match. The query parameter must exist in the
request, in the absence of which the request match fails.</rdfs:comment>
    <rdfs:domain rdf:resource="http://example.org/onto/class/google_compute_region_url_map"/>
    <rdfs:range rdf:resource="http://www.w3.org/2001/XMLSchema#string"/>
  </owl:DatatypeProperty>
  <owl:DatatypeProperty rdf:about="http://example.org/onto/prop/google_compute_region_url_map_present_match">
    <rdfs:label>present_match</rdfs:label>
    <rdfs:comment>Specifies that the queryParameterMatch matches if the request contains the query
parameter, irrespective of whether the parameter has a value or not. Only one of
presentMatch, exactMatch and regexMatch must be set.</rdfs:comment>
    <rdfs:domain rdf:resource="http://example.org/onto/class/google_compute_region_url_map"/>
    <rdfs:range rdf:resource="http://www.w3.org/2001/XMLSchema#string"/>
  </owl:DatatypeProperty>
  <owl:DatatypeProperty rdf:about="http://example.org/onto/prop/google_compute_region_url_map_regex_match">
    <rdfs:label>regex_match</rdfs:label>
    <rdfs:comment>The queryParameterMatch matches if the value of the parameter matches the
regular expression specified by regexMatch. For the regular expression grammar,
please see en.cppreference.com/w/cpp/regex/ecmascript  Only one of presentMatch,
exactMatch and regexMatch must be set.</rdfs:comment>
    <rdfs:domain rdf:resource="http://example.org/onto/class/google_compute_region_url_map"/>
    <rdfs:range rdf:resource="http://www.w3.org/2001/XMLSchema#string"/>
  </owl:DatatypeProperty>
  <owl:DatatypeProperty rdf:about="http://example.org/onto/prop/google_compute_region_url_map_allow_credentials">
    <rdfs:label>allow_credentials</rdfs:label>
    <rdfs:comment>In response to a preflight request, setting this to true indicates that the
actual request can include user credentials. This translates to the Access-
Control-Allow-Credentials header. Defaults to false.</rdfs:comment>
    <rdfs:domain rdf:resource="http://example.org/onto/class/google_compute_region_url_map"/>
    <rdfs:range rdf:resource="http://www.w3.org/2001/XMLSchema#string"/>
  </owl:DatatypeProperty>
  <owl:DatatypeProperty rdf:about="http://example.org/onto/prop/google_compute_region_url_map_allow_headers">
    <rdfs:label>allow_headers</rdfs:label>
    <rdfs:comment>Specifies the content for the Access-Control-Allow-Headers header.</rdfs:comment>
    <rdfs:domain rdf:resource="http://example.org/onto/class/google_compute_region_url_map"/>
    <rdfs:range rdf:resource="http://www.w3.org/2001/XMLSchema#string"/>
  </owl:DatatypeProperty>
  <owl:DatatypeProperty rdf:about="http://example.org/onto/prop/google_compute_region_url_map_allow_methods">
    <rdfs:label>allow_methods</rdfs:label>
    <rdfs:comment>Specifies the content for the Access-Control-Allow-Methods header.</rdfs:comment>
    <rdfs:domain rdf:resource="http://example.org/onto/class/google_compute_region_url_map"/>
    <rdfs:range rdf:resource="http://www.w3.org/2001/XMLSchema#string"/>
  </owl:DatatypeProperty>
  <owl:DatatypeProperty rdf:about="http://example.org/onto/prop/google_compute_region_url_map_allow_origin_regexes">
    <rdfs:label>allow_origin_regexes</rdfs:label>
    <rdfs:comment>Specifies the regular expression patterns that match allowed origins. For
regular expression grammar please see en.cppreference.com/w/cpp/regex/ecmascript
An origin is allowed if it matches either allow_origins or allow_origin_regex.</rdfs:comment>
    <rdfs:domain rdf:resource="http://example.org/onto/class/google_compute_region_url_map"/>
    <rdfs:range rdf:resource="http://www.w3.org/2001/XMLSchema#string"/>
  </owl:DatatypeProperty>
  <owl:DatatypeProperty rdf:about="http://example.org/onto/prop/google_compute_region_url_map_allow_origins">
    <rdfs:label>allow_origins</rdfs:label>
    <rdfs:comment>Specifies the list of origins that will be allowed to do CORS requests. An
origin is allowed if it matches either allow_origins or allow_origin_regex.</rdfs:comment>
    <rdfs:domain rdf:resource="http://example.org/onto/class/google_compute_region_url_map"/>
    <rdfs:range rdf:resource="http://www.w3.org/2001/XMLSchema#string"/>
  </owl:DatatypeProperty>
  <owl:DatatypeProperty rdf:about="http://example.org/onto/prop/google_compute_region_url_map_disabled">
    <rdfs:label>disabled</rdfs:label>
    <rdfs:comment>If true, specifies the CORS policy is disabled.
which indicates that the CORS policy is in effect. Defaults to false.</rdfs:comment>
    <rdfs:domain rdf:resource="http://example.org/onto/class/google_compute_region_url_map"/>
    <rdfs:range rdf:resource="http://www.w3.org/2001/XMLSchema#string"/>
  </owl:DatatypeProperty>
  <owl:DatatypeProperty rdf:about="http://example.org/onto/prop/google_compute_region_url_map_expose_headers">
    <rdfs:label>expose_headers</rdfs:label>
    <rdfs:comment>Specifies the content for the Access-Control-Expose-Headers header.</rdfs:comment>
    <rdfs:domain rdf:resource="http://example.org/onto/class/google_compute_region_url_map"/>
    <rdfs:range rdf:resource="http://www.w3.org/2001/XMLSchema#string"/>
  </owl:DatatypeProperty>
  <owl:DatatypeProperty rdf:about="http://example.org/onto/prop/google_compute_region_url_map_max_age">
    <rdfs:label>max_age</rdfs:label>
    <rdfs:comment>Specifies how long the results of a preflight request can be cached. This
translates to the content for the Access-Control-Max-Age header.</rdfs:comment>
    <rdfs:domain rdf:resource="http://example.org/onto/class/google_compute_region_url_map"/>
    <rdfs:range rdf:resource="http://www.w3.org/2001/XMLSchema#string"/>
  </owl:DatatypeProperty>
  <owl:DatatypeProperty rdf:about="http://example.org/onto/prop/google_compute_region_url_map_http_status">
    <rdfs:label>http_status</rdfs:label>
    <rdfs:comment>The HTTP status code used to abort the request. The value must be between 200
and 599 inclusive.</rdfs:comment>
    <rdfs:domain rdf:resource="http://example.org/onto/class/google_compute_region_url_map"/>
    <rdfs:range rdf:resource="http://www.w3.org/2001/XMLSchema#string"/>
  </owl:DatatypeProperty>
  <owl:DatatypeProperty rdf:about="http://example.org/onto/prop/google_compute_region_url_map_percentage">
    <rdfs:label>percentage</rdfs:label>
    <rdfs:comment>The percentage of traffic (connections/operations/requests) which will be
aborted as part of fault injection. The value must be between 0.0 and 100.0
inclusive.</rdfs:comment>
    <rdfs:domain rdf:resource="http://example.org/onto/class/google_compute_region_url_map"/>
    <rdfs:range rdf:resource="http://www.w3.org/2001/XMLSchema#string"/>
  </owl:DatatypeProperty>
  <owl:DatatypeProperty rdf:about="http://example.org/onto/prop/google_compute_region_url_map_percentage">
    <rdfs:label>percentage</rdfs:label>
    <rdfs:comment>The percentage of traffic (connections/operations/requests) on which delay will
be introduced as part of fault injection. The value must be between 0.0 and
100.0 inclusive.</rdfs:comment>
    <rdfs:domain rdf:resource="http://example.org/onto/class/google_compute_region_url_map"/>
    <rdfs:range rdf:resource="http://www.w3.org/2001/XMLSchema#string"/>
  </owl:DatatypeProperty>
  <owl:DatatypeProperty rdf:about="http://example.org/onto/prop/google_compute_region_url_map_nanos">
    <rdfs:label>nanos</rdfs:label>
    <rdfs:comment>Span of time that's a fraction of a second at nanosecond resolution. Durations
less than one second are represented with a 0 'seconds' field and a positive
'nanos' field. Must be from 0 to 999,999,999 inclusive.</rdfs:comment>
    <rdfs:domain rdf:resource="http://example.org/onto/class/google_compute_region_url_map"/>
    <rdfs:range rdf:resource="http://www.w3.org/2001/XMLSchema#string"/>
  </owl:DatatypeProperty>
  <owl:DatatypeProperty rdf:about="http://example.org/onto/prop/google_compute_region_url_map_seconds">
    <rdfs:label>seconds</rdfs:label>
    <rdfs:comment>Span of time at a resolution of a second. Must be from 0 to 315,576,000,000
inclusive.</rdfs:comment>
    <rdfs:domain rdf:resource="http://example.org/onto/class/google_compute_region_url_map"/>
    <rdfs:range rdf:resource="http://www.w3.org/2001/XMLSchema#string"/>
  </owl:DatatypeProperty>
  <owl:DatatypeProperty rdf:about="http://example.org/onto/prop/google_compute_region_url_map_backend_service">
    <rdfs:label>backend_service</rdfs:label>
    <rdfs:comment>The RegionBackendService resource being mirrored to.</rdfs:comment>
    <rdfs:domain rdf:resource="http://example.org/onto/class/google_compute_region_url_map"/>
    <rdfs:range rdf:resource="http://www.w3.org/2001/XMLSchema#string"/>
  </owl:DatatypeProperty>
  <owl:DatatypeProperty rdf:about="http://example.org/onto/prop/google_compute_region_url_map_num_retries">
    <rdfs:label>num_retries</rdfs:label>
    <rdfs:comment>Specifies the allowed number retries. This number must be > 0.</rdfs:comment>
    <rdfs:domain rdf:resource="http://example.org/onto/class/google_compute_region_url_map"/>
    <rdfs:range rdf:resource="http://www.w3.org/2001/XMLSchema#string"/>
  </owl:DatatypeProperty>
  <owl:DatatypeProperty rdf:about="http://example.org/onto/prop/google_compute_region_url_map_retry_conditions">
    <rdfs:label>retry_conditions</rdfs:label>
    <rdfs:comment>Specifies one or more conditions when this retry rule applies. Valid values are:

* 5xx: Loadbalancer will attempt a retry if the backend service responds with
  any 5xx response code, or if the backend service does not respond at all,
  for example: disconnects, reset, read timeout, connection failure, and refused
  streams.
* gateway-error: Similar to 5xx, but only applies to response codes
  502, 503 or 504.
* connect-failure: Loadbalancer will retry on failures
  connecting to backend services, for example due to connection timeouts.
* retriable-4xx: Loadbalancer will retry for retriable 4xx response codes.
  Currently the only retriable error supported is 409.
* refused-stream: Loadbalancer will retry if the backend service resets the stream with a
  REFUSED_STREAM error code. This reset type indicates that it is safe to retry.
* cancelled: Loadbalancer will retry if the gRPC status code in the response
  header is set to cancelled
* deadline-exceeded: Loadbalancer will retry if the
  gRPC status code in the response header is set to deadline-exceeded
* resource-exhausted: Loadbalancer will retry if the gRPC status code in the response
  header is set to resource-exhausted
* unavailable: Loadbalancer will retry if the gRPC status code in
  the response header is set to unavailable</rdfs:comment>
    <rdfs:domain rdf:resource="http://example.org/onto/class/google_compute_region_url_map"/>
    <rdfs:range rdf:resource="http://www.w3.org/2001/XMLSchema#string"/>
  </owl:DatatypeProperty>
  <owl:DatatypeProperty rdf:about="http://example.org/onto/prop/google_compute_region_url_map_nanos">
    <rdfs:label>nanos</rdfs:label>
    <rdfs:comment>Span of time that's a fraction of a second at nanosecond resolution. Durations
less than one second are represented with a 0 'seconds' field and a positive
'nanos' field. Must be from 0 to 999,999,999 inclusive.</rdfs:comment>
    <rdfs:domain rdf:resource="http://example.org/onto/class/google_compute_region_url_map"/>
    <rdfs:range rdf:resource="http://www.w3.org/2001/XMLSchema#string"/>
  </owl:DatatypeProperty>
  <owl:DatatypeProperty rdf:about="http://example.org/onto/prop/google_compute_region_url_map_seconds">
    <rdfs:label>seconds</rdfs:label>
    <rdfs:comment>Span of time at a resolution of a second. Must be from 0 to 315,576,000,000
inclusive.</rdfs:comment>
    <rdfs:domain rdf:resource="http://example.org/onto/class/google_compute_region_url_map"/>
    <rdfs:range rdf:resource="http://www.w3.org/2001/XMLSchema#string"/>
  </owl:DatatypeProperty>
  <owl:DatatypeProperty rdf:about="http://example.org/onto/prop/google_compute_region_url_map_nanos">
    <rdfs:label>nanos</rdfs:label>
    <rdfs:comment>Span of time that's a fraction of a second at nanosecond resolution. Durations
less than one second are represented with a 0 'seconds' field and a positive
'nanos' field. Must be from 0 to 999,999,999 inclusive.</rdfs:comment>
    <rdfs:domain rdf:resource="http://example.org/onto/class/google_compute_region_url_map"/>
    <rdfs:range rdf:resource="http://www.w3.org/2001/XMLSchema#string"/>
  </owl:DatatypeProperty>
  <owl:DatatypeProperty rdf:about="http://example.org/onto/prop/google_compute_region_url_map_seconds">
    <rdfs:label>seconds</rdfs:label>
    <rdfs:comment>Span of time at a resolution of a second. Must be from 0 to 315,576,000,000
inclusive.</rdfs:comment>
    <rdfs:domain rdf:resource="http://example.org/onto/class/google_compute_region_url_map"/>
    <rdfs:range rdf:resource="http://www.w3.org/2001/XMLSchema#string"/>
  </owl:DatatypeProperty>
  <owl:DatatypeProperty rdf:about="http://example.org/onto/prop/google_compute_region_url_map_host_rewrite">
    <rdfs:label>host_rewrite</rdfs:label>
    <rdfs:comment>Prior to forwarding the request to the selected service, the request's host
header is replaced with contents of hostRewrite. The value must be between 1 and
255 characters.</rdfs:comment>
    <rdfs:domain rdf:resource="http://example.org/onto/class/google_compute_region_url_map"/>
    <rdfs:range rdf:resource="http://www.w3.org/2001/XMLSchema#string"/>
  </owl:DatatypeProperty>
  <owl:DatatypeProperty rdf:about="http://example.org/onto/prop/google_compute_region_url_map_path_prefix_rewrite">
    <rdfs:label>path_prefix_rewrite</rdfs:label>
    <rdfs:comment>Prior to forwarding the request to the selected backend service, the matching
portion of the request's path is replaced by pathPrefixRewrite. The value must
be between 1 and 1024 characters.</rdfs:comment>
    <rdfs:domain rdf:resource="http://example.org/onto/class/google_compute_region_url_map"/>
    <rdfs:range rdf:resource="http://www.w3.org/2001/XMLSchema#string"/>
  </owl:DatatypeProperty>
  <owl:DatatypeProperty rdf:about="http://example.org/onto/prop/google_compute_region_url_map_path_template_rewrite">
    <rdfs:label>path_template_rewrite</rdfs:label>
    <rdfs:comment>Prior to forwarding the request to the selected origin, if the
request matched a pathTemplateMatch, the matching portion of the
request's path is replaced re-written using the pattern specified
by pathTemplateRewrite.

pathTemplateRewrite must be between 1 and 255 characters
(inclusive), must start with a '/', and must only use variables
captured by the route's pathTemplate matchers.

pathTemplateRewrite may only be used when all of a route's
MatchRules specify pathTemplate.

Only one of pathPrefixRewrite and pathTemplateRewrite may be
specified.</rdfs:comment>
    <rdfs:domain rdf:resource="http://example.org/onto/class/google_compute_region_url_map"/>
    <rdfs:range rdf:resource="http://www.w3.org/2001/XMLSchema#string"/>
  </owl:DatatypeProperty>
  <owl:DatatypeProperty rdf:about="http://example.org/onto/prop/google_compute_region_url_map_backend_service">
    <rdfs:label>backend_service</rdfs:label>
    <rdfs:comment>The default RegionBackendService resource. Before
forwarding the request to backendService, the loadbalancer applies any relevant
headerActions specified as part of this backendServiceWeight.</rdfs:comment>
    <rdfs:domain rdf:resource="http://example.org/onto/class/google_compute_region_url_map"/>
    <rdfs:range rdf:resource="http://www.w3.org/2001/XMLSchema#string"/>
  </owl:DatatypeProperty>
  <owl:DatatypeProperty rdf:about="http://example.org/onto/prop/google_compute_region_url_map_weight">
    <rdfs:label>weight</rdfs:label>
    <rdfs:comment>Specifies the fraction of traffic sent to backendService, computed as weight /
(sum of all weightedBackendService weights in routeAction) . The selection of a
backend service is determined only for new traffic. Once a user's request has
been directed to a backendService, subsequent requests will be sent to the same
backendService as determined by the BackendService's session affinity policy.
The value must be between 0 and 1000</rdfs:comment>
    <rdfs:domain rdf:resource="http://example.org/onto/class/google_compute_region_url_map"/>
    <rdfs:range rdf:resource="http://www.w3.org/2001/XMLSchema#string"/>
  </owl:DatatypeProperty>
  <owl:DatatypeProperty rdf:about="http://example.org/onto/prop/google_compute_region_url_map_request_headers_to_remove">
    <rdfs:label>request_headers_to_remove</rdfs:label>
    <rdfs:comment>A list of header names for headers that need to be removed from the request
prior to forwarding the request to the backendService.</rdfs:comment>
    <rdfs:domain rdf:resource="http://example.org/onto/class/google_compute_region_url_map"/>
    <rdfs:range rdf:resource="http://www.w3.org/2001/XMLSchema#string"/>
  </owl:DatatypeProperty>
  <owl:DatatypeProperty rdf:about="http://example.org/onto/prop/google_compute_region_url_map_response_headers_to_remove">
    <rdfs:label>response_headers_to_remove</rdfs:label>
    <rdfs:comment>A list of header names for headers that need to be removed from the response
prior to sending the response back to the client.</rdfs:comment>
    <rdfs:domain rdf:resource="http://example.org/onto/class/google_compute_region_url_map"/>
    <rdfs:range rdf:resource="http://www.w3.org/2001/XMLSchema#string"/>
  </owl:DatatypeProperty>
  <owl:DatatypeProperty rdf:about="http://example.org/onto/prop/google_compute_region_url_map_header_name">
    <rdfs:label>header_name</rdfs:label>
    <rdfs:comment>The name of the header.</rdfs:comment>
    <rdfs:domain rdf:resource="http://example.org/onto/class/google_compute_region_url_map"/>
    <rdfs:range rdf:resource="http://www.w3.org/2001/XMLSchema#string"/>
  </owl:DatatypeProperty>
  <owl:DatatypeProperty rdf:about="http://example.org/onto/prop/google_compute_region_url_map_header_value">
    <rdfs:label>header_value</rdfs:label>
    <rdfs:comment>The value of the header to add.</rdfs:comment>
    <rdfs:domain rdf:resource="http://example.org/onto/class/google_compute_region_url_map"/>
    <rdfs:range rdf:resource="http://www.w3.org/2001/XMLSchema#string"/>
  </owl:DatatypeProperty>
  <owl:DatatypeProperty rdf:about="http://example.org/onto/prop/google_compute_region_url_map_replace">
    <rdfs:label>replace</rdfs:label>
    <rdfs:comment>If false, headerValue is appended to any values that already exist for the
header. If true, headerValue is set for the header, discarding any values that
were set for that header.</rdfs:comment>
    <rdfs:domain rdf:resource="http://example.org/onto/class/google_compute_region_url_map"/>
    <rdfs:range rdf:resource="http://www.w3.org/2001/XMLSchema#string"/>
  </owl:DatatypeProperty>
  <owl:DatatypeProperty rdf:about="http://example.org/onto/prop/google_compute_region_url_map_header_name">
    <rdfs:label>header_name</rdfs:label>
    <rdfs:comment>The name of the header.</rdfs:comment>
    <rdfs:domain rdf:resource="http://example.org/onto/class/google_compute_region_url_map"/>
    <rdfs:range rdf:resource="http://www.w3.org/2001/XMLSchema#string"/>
  </owl:DatatypeProperty>
  <owl:DatatypeProperty rdf:about="http://example.org/onto/prop/google_compute_region_url_map_header_value">
    <rdfs:label>header_value</rdfs:label>
    <rdfs:comment>The value of the header to add.</rdfs:comment>
    <rdfs:domain rdf:resource="http://example.org/onto/class/google_compute_region_url_map"/>
    <rdfs:range rdf:resource="http://www.w3.org/2001/XMLSchema#string"/>
  </owl:DatatypeProperty>
  <owl:DatatypeProperty rdf:about="http://example.org/onto/prop/google_compute_region_url_map_replace">
    <rdfs:label>replace</rdfs:label>
    <rdfs:comment>If false, headerValue is appended to any values that already exist for the
header. If true, headerValue is set for the header, discarding any values that
were set for that header.</rdfs:comment>
    <rdfs:domain rdf:resource="http://example.org/onto/class/google_compute_region_url_map"/>
    <rdfs:range rdf:resource="http://www.w3.org/2001/XMLSchema#string"/>
  </owl:DatatypeProperty>
  <owl:DatatypeProperty rdf:about="http://example.org/onto/prop/google_compute_region_url_map_host_redirect">
    <rdfs:label>host_redirect</rdfs:label>
    <rdfs:comment>The host that will be used in the redirect response instead of the one
that was supplied in the request. The value must be between 1 and 255
characters.</rdfs:comment>
    <rdfs:domain rdf:resource="http://example.org/onto/class/google_compute_region_url_map"/>
    <rdfs:range rdf:resource="http://www.w3.org/2001/XMLSchema#string"/>
  </owl:DatatypeProperty>
  <owl:DatatypeProperty rdf:about="http://example.org/onto/prop/google_compute_region_url_map_https_redirect">
    <rdfs:label>https_redirect</rdfs:label>
    <rdfs:comment>If set to true, the URL scheme in the redirected request is set to https.
If set to false, the URL scheme of the redirected request will remain the
same as that of the request. This must only be set for UrlMaps used in
TargetHttpProxys. Setting this true for TargetHttpsProxy is not
permitted. The default is set to false.</rdfs:comment>
    <rdfs:domain rdf:resource="http://example.org/onto/class/google_compute_region_url_map"/>
    <rdfs:range rdf:resource="http://www.w3.org/2001/XMLSchema#string"/>
  </owl:DatatypeProperty>
  <owl:DatatypeProperty rdf:about="http://example.org/onto/prop/google_compute_region_url_map_path_redirect">
    <rdfs:label>path_redirect</rdfs:label>
    <rdfs:comment>The path that will be used in the redirect response instead of the one
that was supplied in the request. pathRedirect cannot be supplied
together with prefixRedirect. Supply one alone or neither. If neither is
supplied, the path of the original request will be used for the redirect.
The value must be between 1 and 1024 characters.</rdfs:comment>
    <rdfs:domain rdf:resource="http://example.org/onto/class/google_compute_region_url_map"/>
    <rdfs:range rdf:resource="http://www.w3.org/2001/XMLSchema#string"/>
  </owl:DatatypeProperty>
  <owl:DatatypeProperty rdf:about="http://example.org/onto/prop/google_compute_region_url_map_prefix_redirect">
    <rdfs:label>prefix_redirect</rdfs:label>
    <rdfs:comment>The prefix that replaces the prefixMatch specified in the
HttpRouteRuleMatch, retaining the remaining portion of the URL before
redirecting the request. prefixRedirect cannot be supplied together with
pathRedirect. Supply one alone or neither. If neither is supplied, the
path of the original request will be used for the redirect. The value
must be between 1 and 1024 characters.</rdfs:comment>
    <rdfs:domain rdf:resource="http://example.org/onto/class/google_compute_region_url_map"/>
    <rdfs:range rdf:resource="http://www.w3.org/2001/XMLSchema#string"/>
  </owl:DatatypeProperty>
  <owl:DatatypeProperty rdf:about="http://example.org/onto/prop/google_compute_region_url_map_redirect_response_code">
    <rdfs:label>redirect_response_code</rdfs:label>
    <rdfs:comment>The HTTP Status code to use for this RedirectAction. Supported values are:

* MOVED_PERMANENTLY_DEFAULT, which is the default value and corresponds to 301.

* FOUND, which corresponds to 302.

* SEE_OTHER which corresponds to 303.

* TEMPORARY_REDIRECT, which corresponds to 307. In this case, the request method
will be retained.

* PERMANENT_REDIRECT, which corresponds to 308. In this case,
the request method will be retained. Possible values: ["FOUND", "MOVED_PERMANENTLY_DEFAULT", "PERMANENT_REDIRECT", "SEE_OTHER", "TEMPORARY_REDIRECT"]</rdfs:comment>
    <rdfs:domain rdf:resource="http://example.org/onto/class/google_compute_region_url_map"/>
    <rdfs:range rdf:resource="http://www.w3.org/2001/XMLSchema#string"/>
  </owl:DatatypeProperty>
  <owl:DatatypeProperty rdf:about="http://example.org/onto/prop/google_compute_region_url_map_strip_query">
    <rdfs:label>strip_query</rdfs:label>
    <rdfs:comment>If set to true, any accompanying query portion of the original URL is
removed prior to redirecting the request. If set to false, the query
portion of the original URL is retained. The default value is false.</rdfs:comment>
    <rdfs:domain rdf:resource="http://example.org/onto/class/google_compute_region_url_map"/>
    <rdfs:range rdf:resource="http://www.w3.org/2001/XMLSchema#string"/>
  </owl:DatatypeProperty>
  <owl:DatatypeProperty rdf:about="http://example.org/onto/prop/google_compute_region_url_map_description">
    <rdfs:label>description</rdfs:label>
    <rdfs:comment>Description of this test case.</rdfs:comment>
    <rdfs:domain rdf:resource="http://example.org/onto/class/google_compute_region_url_map"/>
    <rdfs:range rdf:resource="http://www.w3.org/2001/XMLSchema#string"/>
  </owl:DatatypeProperty>
  <owl:DatatypeProperty rdf:about="http://example.org/onto/prop/google_compute_region_url_map_host">
    <rdfs:label>host</rdfs:label>
    <rdfs:comment>Host portion of the URL.</rdfs:comment>
    <rdfs:domain rdf:resource="http://example.org/onto/class/google_compute_region_url_map"/>
    <rdfs:range rdf:resource="http://www.w3.org/2001/XMLSchema#string"/>
  </owl:DatatypeProperty>
  <owl:DatatypeProperty rdf:about="http://example.org/onto/prop/google_compute_region_url_map_path">
    <rdfs:label>path</rdfs:label>
    <rdfs:comment>Path portion of the URL.</rdfs:comment>
    <rdfs:domain rdf:resource="http://example.org/onto/class/google_compute_region_url_map"/>
    <rdfs:range rdf:resource="http://www.w3.org/2001/XMLSchema#string"/>
  </owl:DatatypeProperty>
  <owl:DatatypeProperty rdf:about="http://example.org/onto/prop/google_compute_region_url_map_service">
    <rdfs:label>service</rdfs:label>
    <rdfs:comment>A reference to expected RegionBackendService resource the given URL should be mapped to.</rdfs:comment>
    <rdfs:domain rdf:resource="http://example.org/onto/class/google_compute_region_url_map"/>
    <rdfs:range rdf:resource="http://www.w3.org/2001/XMLSchema#string"/>
  </owl:DatatypeProperty>
  <owl:DatatypeProperty rdf:about="http://example.org/onto/prop/google_compute_region_url_map_create">
    <rdfs:label>create</rdfs:label>
    <rdfs:domain rdf:resource="http://example.org/onto/class/google_compute_region_url_map"/>
    <rdfs:range rdf:resource="http://www.w3.org/2001/XMLSchema#string"/>
  </owl:DatatypeProperty>
  <owl:DatatypeProperty rdf:about="http://example.org/onto/prop/google_compute_region_url_map_delete">
    <rdfs:label>delete</rdfs:label>
    <rdfs:domain rdf:resource="http://example.org/onto/class/google_compute_region_url_map"/>
    <rdfs:range rdf:resource="http://www.w3.org/2001/XMLSchema#string"/>
  </owl:DatatypeProperty>
  <owl:DatatypeProperty rdf:about="http://example.org/onto/prop/google_compute_region_url_map_update">
    <rdfs:label>update</rdfs:label>
    <rdfs:domain rdf:resource="http://example.org/onto/class/google_compute_region_url_map"/>
    <rdfs:range rdf:resource="http://www.w3.org/2001/XMLSchema#string"/>
  </owl:DatatypeProperty>
</rdf:RDF>
