<?xml version="1.0" encoding="UTF-8"?>
<rdf:RDF
  xmlns:rdf="http://www.w3.org/1999/02/22-rdf-syntax-ns#"
  xmlns:rdfs="http://www.w3.org/2000/01/rdf-schema#"
  xmlns:owl="http://www.w3.org/2002/07/owl#"
  xmlns:xsd="http://www.w3.org/2001/XMLSchema#"
  xml:base="http://example.org/onto/">
  <owl:Class rdf:about="http://example.org/onto/class/google_assured_workloads_workload">
    <rdfs:label>google_assured_workloads_workload</rdfs:label>
    <rdfs:comment>#
#     ***     AUTO GENERATED CODE    ***    Type: DCL     ***
#
# ----------------------------------------------------------------------------
#
#     This file is managed by Magic Modules (https:#github.com/GoogleCloudPlatform/magic-modules)
#     and is based on the DCL (https:#github.com/GoogleCloudPlatform/declarative-resource-client-library).
#     Changes will need to be made to the DCL or Magic Modules instead of here.
#
#     We are not currently able to accept contributions to this file. If changes
#     are required, please file an issue at https:#github.com/hashicorp/terraform-provider-google/issues/new/choose
#
# ----------------------------------------------------------------------------
subcategory: "AssuredWorkloads"
description: |-
  The AssuredWorkloads Workload resource
---</rdfs:comment>
  </owl:Class>
  <owl:DatatypeProperty rdf:about="http://example.org/onto/prop/google_assured_workloads_workload_billing_account">
    <rdfs:label>billing_account</rdfs:label>
    <rdfs:comment>Optional. Input only. The billing account used for the resources which are direct children of workload. This billing account is initially associated with the resources created as part of Workload creation. After the initial creation of these resources, the customer can change the assigned billing account. The resource name has the form `billingAccounts/{billing_account_id}`. For example, `billingAccounts/012345-567890-ABCDEF`.</rdfs:comment>
    <rdfs:domain rdf:resource="http://example.org/onto/class/google_assured_workloads_workload"/>
    <rdfs:range rdf:resource="http://www.w3.org/2001/XMLSchema#string"/>
  </owl:DatatypeProperty>
  <owl:DatatypeProperty rdf:about="http://example.org/onto/prop/google_assured_workloads_workload_compliance_regime">
    <rdfs:label>compliance_regime</rdfs:label>
    <rdfs:comment>Required. Immutable. Compliance Regime associated with this workload. Possible values: COMPLIANCE_REGIME_UNSPECIFIED, IL4, CJIS, FEDRAMP_HIGH, FEDRAMP_MODERATE, US_REGIONAL_ACCESS, HIPAA, HITRUST, EU_REGIONS_AND_SUPPORT, CA_REGIONS_AND_SUPPORT, ITAR, AU_REGIONS_AND_US_SUPPORT, ASSURED_WORKLOADS_FOR_PARTNERS, ISR_REGIONS, ISR_REGIONS_AND_SUPPORT, CA_PROTECTED_B, IL5, IL2, JP_REGIONS_AND_SUPPORT, KSA_REGIONS_AND_SUPPORT_WITH_SOVEREIGNTY_CONTROLS, REGIONAL_CONTROLS, HEALTHCARE_AND_LIFE_SCIENCES_CONTROLS, HEALTHCARE_AND_LIFE_SCIENCES_CONTROLS_US_SUPPORT, IRS_1075</rdfs:comment>
    <rdfs:domain rdf:resource="http://example.org/onto/class/google_assured_workloads_workload"/>
    <rdfs:range rdf:resource="http://www.w3.org/2001/XMLSchema#string"/>
  </owl:DatatypeProperty>
  <owl:DatatypeProperty rdf:about="http://example.org/onto/prop/google_assured_workloads_workload_compliance_status">
    <rdfs:label>compliance_status</rdfs:label>
    <rdfs:comment>Output only. Count of active Violations in the Workload.</rdfs:comment>
    <rdfs:domain rdf:resource="http://example.org/onto/class/google_assured_workloads_workload"/>
    <rdfs:range rdf:resource="http://www.w3.org/2001/XMLSchema#string"/>
  </owl:DatatypeProperty>
  <owl:DatatypeProperty rdf:about="http://example.org/onto/prop/google_assured_workloads_workload_compliant_but_disallowed_services">
    <rdfs:label>compliant_but_disallowed_services</rdfs:label>
    <rdfs:comment>Output only. Urls for services which are compliant for this Assured Workload, but which are currently disallowed by the ResourceUsageRestriction org policy. Invoke workloads.restrictAllowedResources endpoint to allow your project developers to use these services in their environment.</rdfs:comment>
    <rdfs:domain rdf:resource="http://example.org/onto/class/google_assured_workloads_workload"/>
    <rdfs:range rdf:resource="http://www.w3.org/2001/XMLSchema#string"/>
  </owl:DatatypeProperty>
  <owl:DatatypeProperty rdf:about="http://example.org/onto/prop/google_assured_workloads_workload_create_time">
    <rdfs:label>create_time</rdfs:label>
    <rdfs:comment>Output only. Immutable. The Workload creation timestamp.</rdfs:comment>
    <rdfs:domain rdf:resource="http://example.org/onto/class/google_assured_workloads_workload"/>
    <rdfs:range rdf:resource="http://www.w3.org/2001/XMLSchema#string"/>
  </owl:DatatypeProperty>
  <owl:DatatypeProperty rdf:about="http://example.org/onto/prop/google_assured_workloads_workload_display_name">
    <rdfs:label>display_name</rdfs:label>
    <rdfs:comment>Required. The user-assigned display name of the Workload. When present it must be between 4 to 30 characters. Allowed characters are: lowercase and uppercase letters, numbers, hyphen, and spaces. Example: My Workload</rdfs:comment>
    <rdfs:domain rdf:resource="http://example.org/onto/class/google_assured_workloads_workload"/>
    <rdfs:range rdf:resource="http://www.w3.org/2001/XMLSchema#string"/>
  </owl:DatatypeProperty>
  <owl:DatatypeProperty rdf:about="http://example.org/onto/prop/google_assured_workloads_workload_effective_labels">
    <rdfs:label>effective_labels</rdfs:label>
    <rdfs:comment>All of labels (key/value pairs) present on the resource in GCP, including the labels configured through Terraform, other clients and services.</rdfs:comment>
    <rdfs:domain rdf:resource="http://example.org/onto/class/google_assured_workloads_workload"/>
    <rdfs:range rdf:resource="http://www.w3.org/2001/XMLSchema#string"/>
  </owl:DatatypeProperty>
  <owl:DatatypeProperty rdf:about="http://example.org/onto/prop/google_assured_workloads_workload_ekm_provisioning_response">
    <rdfs:label>ekm_provisioning_response</rdfs:label>
    <rdfs:comment>Optional. Represents the Ekm Provisioning State of the given workload.</rdfs:comment>
    <rdfs:domain rdf:resource="http://example.org/onto/class/google_assured_workloads_workload"/>
    <rdfs:range rdf:resource="http://www.w3.org/2001/XMLSchema#string"/>
  </owl:DatatypeProperty>
  <owl:DatatypeProperty rdf:about="http://example.org/onto/prop/google_assured_workloads_workload_enable_sovereign_controls">
    <rdfs:label>enable_sovereign_controls</rdfs:label>
    <rdfs:comment>Optional. Indicates the sovereignty status of the given workload. Currently meant to be used by Europe/Canada customers.</rdfs:comment>
    <rdfs:domain rdf:resource="http://example.org/onto/class/google_assured_workloads_workload"/>
    <rdfs:range rdf:resource="http://www.w3.org/2001/XMLSchema#string"/>
  </owl:DatatypeProperty>
  <owl:DatatypeProperty rdf:about="http://example.org/onto/prop/google_assured_workloads_workload_id">
    <rdfs:label>id</rdfs:label>
    <rdfs:domain rdf:resource="http://example.org/onto/class/google_assured_workloads_workload"/>
    <rdfs:range rdf:resource="http://www.w3.org/2001/XMLSchema#string"/>
  </owl:DatatypeProperty>
  <owl:DatatypeProperty rdf:about="http://example.org/onto/prop/google_assured_workloads_workload_kaj_enrollment_state">
    <rdfs:label>kaj_enrollment_state</rdfs:label>
    <rdfs:comment>Output only. Represents the KAJ enrollment state of the given workload. Possible values: KAJ_ENROLLMENT_STATE_UNSPECIFIED, KAJ_ENROLLMENT_STATE_PENDING, KAJ_ENROLLMENT_STATE_COMPLETE</rdfs:comment>
    <rdfs:domain rdf:resource="http://example.org/onto/class/google_assured_workloads_workload"/>
    <rdfs:range rdf:resource="http://www.w3.org/2001/XMLSchema#string"/>
  </owl:DatatypeProperty>
  <owl:DatatypeProperty rdf:about="http://example.org/onto/prop/google_assured_workloads_workload_labels">
    <rdfs:label>labels</rdfs:label>
    <rdfs:comment>Optional. Labels applied to the workload.

**Note**: This field is non-authoritative, and will only manage the labels present in your configuration.
Please refer to the field `effective_labels` for all of the labels present on the resource.</rdfs:comment>
    <rdfs:domain rdf:resource="http://example.org/onto/class/google_assured_workloads_workload"/>
    <rdfs:range rdf:resource="http://www.w3.org/2001/XMLSchema#string"/>
  </owl:DatatypeProperty>
  <owl:DatatypeProperty rdf:about="http://example.org/onto/prop/google_assured_workloads_workload_location">
    <rdfs:label>location</rdfs:label>
    <rdfs:comment>The location for the resource</rdfs:comment>
    <rdfs:domain rdf:resource="http://example.org/onto/class/google_assured_workloads_workload"/>
    <rdfs:range rdf:resource="http://www.w3.org/2001/XMLSchema#string"/>
  </owl:DatatypeProperty>
  <owl:DatatypeProperty rdf:about="http://example.org/onto/prop/google_assured_workloads_workload_name">
    <rdfs:label>name</rdfs:label>
    <rdfs:comment>Output only. The resource name of the workload.</rdfs:comment>
    <rdfs:domain rdf:resource="http://example.org/onto/class/google_assured_workloads_workload"/>
    <rdfs:range rdf:resource="http://www.w3.org/2001/XMLSchema#string"/>
  </owl:DatatypeProperty>
  <owl:DatatypeProperty rdf:about="http://example.org/onto/prop/google_assured_workloads_workload_organization">
    <rdfs:label>organization</rdfs:label>
    <rdfs:comment>The organization for the resource</rdfs:comment>
    <rdfs:domain rdf:resource="http://example.org/onto/class/google_assured_workloads_workload"/>
    <rdfs:range rdf:resource="http://www.w3.org/2001/XMLSchema#string"/>
  </owl:DatatypeProperty>
  <owl:DatatypeProperty rdf:about="http://example.org/onto/prop/google_assured_workloads_workload_partner">
    <rdfs:label>partner</rdfs:label>
    <rdfs:comment>Optional. Partner regime associated with this workload. Possible values: PARTNER_UNSPECIFIED, LOCAL_CONTROLS_BY_S3NS, SOVEREIGN_CONTROLS_BY_T_SYSTEMS, SOVEREIGN_CONTROLS_BY_SIA_MINSAIT, SOVEREIGN_CONTROLS_BY_PSN, SOVEREIGN_CONTROLS_BY_CNTXT, SOVEREIGN_CONTROLS_BY_CNTXT_NO_EKM</rdfs:comment>
    <rdfs:domain rdf:resource="http://example.org/onto/class/google_assured_workloads_workload"/>
    <rdfs:range rdf:resource="http://www.w3.org/2001/XMLSchema#string"/>
  </owl:DatatypeProperty>
  <owl:DatatypeProperty rdf:about="http://example.org/onto/prop/google_assured_workloads_workload_partner_services_billing_account">
    <rdfs:label>partner_services_billing_account</rdfs:label>
    <rdfs:comment>Optional. Input only. Billing account necessary for purchasing services from Sovereign Partners. This field is required for creating SIA/PSN/CNTXT partner workloads. The caller should have 'billing.resourceAssociations.create' IAM permission on this billing-account. The format of this string is billingAccounts/AAAAAA-BBBBBB-CCCCCC.</rdfs:comment>
    <rdfs:domain rdf:resource="http://example.org/onto/class/google_assured_workloads_workload"/>
    <rdfs:range rdf:resource="http://www.w3.org/2001/XMLSchema#string"/>
  </owl:DatatypeProperty>
  <owl:DatatypeProperty rdf:about="http://example.org/onto/prop/google_assured_workloads_workload_provisioned_resources_parent">
    <rdfs:label>provisioned_resources_parent</rdfs:label>
    <rdfs:comment>Input only. The parent resource for the resources managed by this Assured Workload. May be either empty or a folder resource which is a child of the Workload parent. If not specified all resources are created under the parent organization. Format: folders/{folder_id}</rdfs:comment>
    <rdfs:domain rdf:resource="http://example.org/onto/class/google_assured_workloads_workload"/>
    <rdfs:range rdf:resource="http://www.w3.org/2001/XMLSchema#string"/>
  </owl:DatatypeProperty>
  <owl:DatatypeProperty rdf:about="http://example.org/onto/prop/google_assured_workloads_workload_resources">
    <rdfs:label>resources</rdfs:label>
    <rdfs:comment>Output only. The resources associated with this workload. These resources will be created when creating the workload. If any of the projects already exist, the workload creation will fail. Always read only.</rdfs:comment>
    <rdfs:domain rdf:resource="http://example.org/onto/class/google_assured_workloads_workload"/>
    <rdfs:range rdf:resource="http://www.w3.org/2001/XMLSchema#string"/>
  </owl:DatatypeProperty>
  <owl:DatatypeProperty rdf:about="http://example.org/onto/prop/google_assured_workloads_workload_saa_enrollment_response">
    <rdfs:label>saa_enrollment_response</rdfs:label>
    <rdfs:comment>Output only. Represents the SAA enrollment response of the given workload. SAA enrollment response is queried during workloads.get call. In failure cases, user friendly error message is shown in SAA details page.</rdfs:comment>
    <rdfs:domain rdf:resource="http://example.org/onto/class/google_assured_workloads_workload"/>
    <rdfs:range rdf:resource="http://www.w3.org/2001/XMLSchema#string"/>
  </owl:DatatypeProperty>
  <owl:DatatypeProperty rdf:about="http://example.org/onto/prop/google_assured_workloads_workload_terraform_labels">
    <rdfs:label>terraform_labels</rdfs:label>
    <rdfs:comment>The combination of labels configured directly on the resource and default labels configured on the provider.</rdfs:comment>
    <rdfs:domain rdf:resource="http://example.org/onto/class/google_assured_workloads_workload"/>
    <rdfs:range rdf:resource="http://www.w3.org/2001/XMLSchema#string"/>
  </owl:DatatypeProperty>
  <owl:DatatypeProperty rdf:about="http://example.org/onto/prop/google_assured_workloads_workload_violation_notifications_enabled">
    <rdfs:label>violation_notifications_enabled</rdfs:label>
    <rdfs:comment>Optional. Indicates whether the e-mail notification for a violation is enabled for a workload. This value will be by default True, and if not present will be considered as true. This should only be updated via updateWorkload call. Any Changes to this field during the createWorkload call will not be honored. This will always be true while creating the workload.</rdfs:comment>
    <rdfs:domain rdf:resource="http://example.org/onto/class/google_assured_workloads_workload"/>
    <rdfs:range rdf:resource="http://www.w3.org/2001/XMLSchema#string"/>
  </owl:DatatypeProperty>
  <owl:DatatypeProperty rdf:about="http://example.org/onto/prop/google_assured_workloads_workload_next_rotation_time">
    <rdfs:label>next_rotation_time</rdfs:label>
    <rdfs:comment>Required. Input only. Immutable. The time at which the Key Management Service will automatically create a new version of the crypto key and mark it as the primary.</rdfs:comment>
    <rdfs:domain rdf:resource="http://example.org/onto/class/google_assured_workloads_workload"/>
    <rdfs:range rdf:resource="http://www.w3.org/2001/XMLSchema#string"/>
  </owl:DatatypeProperty>
  <owl:DatatypeProperty rdf:about="http://example.org/onto/prop/google_assured_workloads_workload_rotation_period">
    <rdfs:label>rotation_period</rdfs:label>
    <rdfs:comment>Required. Input only. Immutable. will be advanced by this period when the Key Management Service automatically rotates a key. Must be at least 24 hours and at most 876,000 hours.</rdfs:comment>
    <rdfs:domain rdf:resource="http://example.org/onto/class/google_assured_workloads_workload"/>
    <rdfs:range rdf:resource="http://www.w3.org/2001/XMLSchema#string"/>
  </owl:DatatypeProperty>
  <owl:DatatypeProperty rdf:about="http://example.org/onto/prop/google_assured_workloads_workload_assured_workloads_monitoring">
    <rdfs:label>assured_workloads_monitoring</rdfs:label>
    <rdfs:comment>Optional. Allow partner to view violation alerts.</rdfs:comment>
    <rdfs:domain rdf:resource="http://example.org/onto/class/google_assured_workloads_workload"/>
    <rdfs:range rdf:resource="http://www.w3.org/2001/XMLSchema#string"/>
  </owl:DatatypeProperty>
  <owl:DatatypeProperty rdf:about="http://example.org/onto/prop/google_assured_workloads_workload_data_logs_viewer">
    <rdfs:label>data_logs_viewer</rdfs:label>
    <rdfs:comment>Allow the partner to view inspectability logs and monitoring violations.</rdfs:comment>
    <rdfs:domain rdf:resource="http://example.org/onto/class/google_assured_workloads_workload"/>
    <rdfs:range rdf:resource="http://www.w3.org/2001/XMLSchema#string"/>
  </owl:DatatypeProperty>
  <owl:DatatypeProperty rdf:about="http://example.org/onto/prop/google_assured_workloads_workload_service_access_approver">
    <rdfs:label>service_access_approver</rdfs:label>
    <rdfs:comment>Optional. Allow partner to view access approval logs.</rdfs:comment>
    <rdfs:domain rdf:resource="http://example.org/onto/class/google_assured_workloads_workload"/>
    <rdfs:range rdf:resource="http://www.w3.org/2001/XMLSchema#string"/>
  </owl:DatatypeProperty>
  <owl:DatatypeProperty rdf:about="http://example.org/onto/prop/google_assured_workloads_workload_display_name">
    <rdfs:label>display_name</rdfs:label>
    <rdfs:comment>User-assigned resource display name. If not empty it will be used to create a resource with the specified name.</rdfs:comment>
    <rdfs:domain rdf:resource="http://example.org/onto/class/google_assured_workloads_workload"/>
    <rdfs:range rdf:resource="http://www.w3.org/2001/XMLSchema#string"/>
  </owl:DatatypeProperty>
  <owl:DatatypeProperty rdf:about="http://example.org/onto/prop/google_assured_workloads_workload_resource_id">
    <rdfs:label>resource_id</rdfs:label>
    <rdfs:comment>Resource identifier. For a project this represents projectId. If the project is already taken, the workload creation will fail. For KeyRing, this represents the keyring_id. For a folder, don't set this value as folder_id is assigned by Google.</rdfs:comment>
    <rdfs:domain rdf:resource="http://example.org/onto/class/google_assured_workloads_workload"/>
    <rdfs:range rdf:resource="http://www.w3.org/2001/XMLSchema#string"/>
  </owl:DatatypeProperty>
  <owl:DatatypeProperty rdf:about="http://example.org/onto/prop/google_assured_workloads_workload_resource_type">
    <rdfs:label>resource_type</rdfs:label>
    <rdfs:comment>Indicates the type of resource. This field should be specified to correspond the id to the right project type (CONSUMER_PROJECT or ENCRYPTION_KEYS_PROJECT) Possible values: RESOURCE_TYPE_UNSPECIFIED, CONSUMER_PROJECT, ENCRYPTION_KEYS_PROJECT, KEYRING, CONSUMER_FOLDER</rdfs:comment>
    <rdfs:domain rdf:resource="http://example.org/onto/class/google_assured_workloads_workload"/>
    <rdfs:range rdf:resource="http://www.w3.org/2001/XMLSchema#string"/>
  </owl:DatatypeProperty>
  <owl:DatatypeProperty rdf:about="http://example.org/onto/prop/google_assured_workloads_workload_create">
    <rdfs:label>create</rdfs:label>
    <rdfs:domain rdf:resource="http://example.org/onto/class/google_assured_workloads_workload"/>
    <rdfs:range rdf:resource="http://www.w3.org/2001/XMLSchema#string"/>
  </owl:DatatypeProperty>
  <owl:DatatypeProperty rdf:about="http://example.org/onto/prop/google_assured_workloads_workload_delete">
    <rdfs:label>delete</rdfs:label>
    <rdfs:domain rdf:resource="http://example.org/onto/class/google_assured_workloads_workload"/>
    <rdfs:range rdf:resource="http://www.w3.org/2001/XMLSchema#string"/>
  </owl:DatatypeProperty>
  <owl:DatatypeProperty rdf:about="http://example.org/onto/prop/google_assured_workloads_workload_update">
    <rdfs:label>update</rdfs:label>
    <rdfs:domain rdf:resource="http://example.org/onto/class/google_assured_workloads_workload"/>
    <rdfs:range rdf:resource="http://www.w3.org/2001/XMLSchema#string"/>
  </owl:DatatypeProperty>
  <owl:DatatypeProperty rdf:about="http://example.org/onto/prop/google_assured_workloads_workload_kaj_enrollment_type">
    <rdfs:label>kaj_enrollment_type</rdfs:label>
    <rdfs:comment>Indicates type of KAJ enrollment for the workload. Currently, only specifiying KEY_ACCESS_TRANSPARENCY_OFF is implemented to not enroll in KAT-level KAJ enrollment for Regional Controls workloads. Possible values: KAJ_ENROLLMENT_TYPE_UNSPECIFIED, FULL_KAJ, EKM_ONLY, KEY_ACCESS_TRANSPARENCY_OFF</rdfs:comment>
    <rdfs:domain rdf:resource="http://example.org/onto/class/google_assured_workloads_workload"/>
    <rdfs:range rdf:resource="http://www.w3.org/2001/XMLSchema#string"/>
  </owl:DatatypeProperty>
</rdf:RDF>
