<?xml version="1.0" encoding="UTF-8"?>
<rdf:RDF
  xmlns:rdf="http://www.w3.org/1999/02/22-rdf-syntax-ns#"
  xmlns:rdfs="http://www.w3.org/2000/01/rdf-schema#"
  xmlns:owl="http://www.w3.org/2002/07/owl#"
  xmlns:xsd="http://www.w3.org/2001/XMLSchema#"
  xml:base="http://example.org/onto/">
  <owl:Class rdf:about="http://example.org/onto/class/google_vmwareengine_network_peering">
    <rdfs:label>google_vmwareengine_network_peering</rdfs:label>
    <rdfs:comment>#
#     ***     AUTO GENERATED CODE    ***    Type: MMv1     ***
#
# ----------------------------------------------------------------------------
#
#     This code is generated by Magic Modules using the following:
#
#     Configuration: https:#github.com/GoogleCloudPlatform/magic-modules/tree/main/mmv1/products/vmwareengine/NetworkPeering.yaml
#     Template:      https:#github.com/GoogleCloudPlatform/magic-modules/tree/main/mmv1/templates/terraform/resource.html.markdown.tmpl
#
#     DO NOT EDIT this file directly. Any changes made to this file will be
#     overwritten during the next generation cycle.
#
# ----------------------------------------------------------------------------
subcategory: "Cloud VMware Engine"
description: |-
  Represents a network peering resource.
---</rdfs:comment>
  </owl:Class>
  <owl:DatatypeProperty rdf:about="http://example.org/onto/prop/google_vmwareengine_network_peering_create_time">
    <rdfs:label>create_time</rdfs:label>
    <rdfs:comment>Creation time of this resource.
A timestamp in RFC3339 UTC "Zulu" format, with nanosecond resolution and
up to nine fractional digits. Examples: "2014-10-02T15:01:23Z" and "2014-10-02T15:01:23.045123456Z".</rdfs:comment>
    <rdfs:domain rdf:resource="http://example.org/onto/class/google_vmwareengine_network_peering"/>
    <rdfs:range rdf:resource="http://www.w3.org/2001/XMLSchema#string"/>
  </owl:DatatypeProperty>
  <owl:DatatypeProperty rdf:about="http://example.org/onto/prop/google_vmwareengine_network_peering_description">
    <rdfs:label>description</rdfs:label>
    <rdfs:comment>User-provided description for this network peering.</rdfs:comment>
    <rdfs:domain rdf:resource="http://example.org/onto/class/google_vmwareengine_network_peering"/>
    <rdfs:range rdf:resource="http://www.w3.org/2001/XMLSchema#string"/>
  </owl:DatatypeProperty>
  <owl:DatatypeProperty rdf:about="http://example.org/onto/prop/google_vmwareengine_network_peering_export_custom_routes">
    <rdfs:label>export_custom_routes</rdfs:label>
    <rdfs:comment>True if custom routes are exported to the peered network; false otherwise.</rdfs:comment>
    <rdfs:domain rdf:resource="http://example.org/onto/class/google_vmwareengine_network_peering"/>
    <rdfs:range rdf:resource="http://www.w3.org/2001/XMLSchema#string"/>
  </owl:DatatypeProperty>
  <owl:DatatypeProperty rdf:about="http://example.org/onto/prop/google_vmwareengine_network_peering_export_custom_routes_with_public_ip">
    <rdfs:label>export_custom_routes_with_public_ip</rdfs:label>
    <rdfs:comment>True if all subnet routes with a public IP address range are exported; false otherwise.</rdfs:comment>
    <rdfs:domain rdf:resource="http://example.org/onto/class/google_vmwareengine_network_peering"/>
    <rdfs:range rdf:resource="http://www.w3.org/2001/XMLSchema#string"/>
  </owl:DatatypeProperty>
  <owl:DatatypeProperty rdf:about="http://example.org/onto/prop/google_vmwareengine_network_peering_id">
    <rdfs:label>id</rdfs:label>
    <rdfs:domain rdf:resource="http://example.org/onto/class/google_vmwareengine_network_peering"/>
    <rdfs:range rdf:resource="http://www.w3.org/2001/XMLSchema#string"/>
  </owl:DatatypeProperty>
  <owl:DatatypeProperty rdf:about="http://example.org/onto/prop/google_vmwareengine_network_peering_import_custom_routes">
    <rdfs:label>import_custom_routes</rdfs:label>
    <rdfs:comment>True if custom routes are imported from the peered network; false otherwise.</rdfs:comment>
    <rdfs:domain rdf:resource="http://example.org/onto/class/google_vmwareengine_network_peering"/>
    <rdfs:range rdf:resource="http://www.w3.org/2001/XMLSchema#string"/>
  </owl:DatatypeProperty>
  <owl:DatatypeProperty rdf:about="http://example.org/onto/prop/google_vmwareengine_network_peering_import_custom_routes_with_public_ip">
    <rdfs:label>import_custom_routes_with_public_ip</rdfs:label>
    <rdfs:comment>True if custom routes are imported from the peered network; false otherwise.</rdfs:comment>
    <rdfs:domain rdf:resource="http://example.org/onto/class/google_vmwareengine_network_peering"/>
    <rdfs:range rdf:resource="http://www.w3.org/2001/XMLSchema#string"/>
  </owl:DatatypeProperty>
  <owl:DatatypeProperty rdf:about="http://example.org/onto/prop/google_vmwareengine_network_peering_name">
    <rdfs:label>name</rdfs:label>
    <rdfs:comment>The ID of the Network Peering.</rdfs:comment>
    <rdfs:domain rdf:resource="http://example.org/onto/class/google_vmwareengine_network_peering"/>
    <rdfs:range rdf:resource="http://www.w3.org/2001/XMLSchema#string"/>
  </owl:DatatypeProperty>
  <owl:DatatypeProperty rdf:about="http://example.org/onto/prop/google_vmwareengine_network_peering_peer_network">
    <rdfs:label>peer_network</rdfs:label>
    <rdfs:comment>The relative resource name of the network to peer with a standard VMware Engine network.
The provided network can be a consumer VPC network or another standard VMware Engine network.</rdfs:comment>
    <rdfs:domain rdf:resource="http://example.org/onto/class/google_vmwareengine_network_peering"/>
    <rdfs:range rdf:resource="http://www.w3.org/2001/XMLSchema#string"/>
  </owl:DatatypeProperty>
  <owl:DatatypeProperty rdf:about="http://example.org/onto/prop/google_vmwareengine_network_peering_peer_network_type">
    <rdfs:label>peer_network_type</rdfs:label>
    <rdfs:comment>The type of the network to peer with the VMware Engine network. Possible values: ["STANDARD", "VMWARE_ENGINE_NETWORK", "PRIVATE_SERVICES_ACCESS", "NETAPP_CLOUD_VOLUMES", "THIRD_PARTY_SERVICE", "DELL_POWERSCALE", "GOOGLE_CLOUD_NETAPP_VOLUMES"]</rdfs:comment>
    <rdfs:domain rdf:resource="http://example.org/onto/class/google_vmwareengine_network_peering"/>
    <rdfs:range rdf:resource="http://www.w3.org/2001/XMLSchema#string"/>
  </owl:DatatypeProperty>
  <owl:DatatypeProperty rdf:about="http://example.org/onto/prop/google_vmwareengine_network_peering_project">
    <rdfs:label>project</rdfs:label>
    <rdfs:domain rdf:resource="http://example.org/onto/class/google_vmwareengine_network_peering"/>
    <rdfs:range rdf:resource="http://www.w3.org/2001/XMLSchema#string"/>
  </owl:DatatypeProperty>
  <owl:DatatypeProperty rdf:about="http://example.org/onto/prop/google_vmwareengine_network_peering_state">
    <rdfs:label>state</rdfs:label>
    <rdfs:comment>State of the network peering.
This field has a value of 'ACTIVE' when there's a matching configuration in the peer network.
New values may be added to this enum when appropriate.</rdfs:comment>
    <rdfs:domain rdf:resource="http://example.org/onto/class/google_vmwareengine_network_peering"/>
    <rdfs:range rdf:resource="http://www.w3.org/2001/XMLSchema#string"/>
  </owl:DatatypeProperty>
  <owl:DatatypeProperty rdf:about="http://example.org/onto/prop/google_vmwareengine_network_peering_state_details">
    <rdfs:label>state_details</rdfs:label>
    <rdfs:comment>Details about the current state of the network peering.</rdfs:comment>
    <rdfs:domain rdf:resource="http://example.org/onto/class/google_vmwareengine_network_peering"/>
    <rdfs:range rdf:resource="http://www.w3.org/2001/XMLSchema#string"/>
  </owl:DatatypeProperty>
  <owl:DatatypeProperty rdf:about="http://example.org/onto/prop/google_vmwareengine_network_peering_uid">
    <rdfs:label>uid</rdfs:label>
    <rdfs:comment>System-generated unique identifier for the resource.</rdfs:comment>
    <rdfs:domain rdf:resource="http://example.org/onto/class/google_vmwareengine_network_peering"/>
    <rdfs:range rdf:resource="http://www.w3.org/2001/XMLSchema#string"/>
  </owl:DatatypeProperty>
  <owl:DatatypeProperty rdf:about="http://example.org/onto/prop/google_vmwareengine_network_peering_update_time">
    <rdfs:label>update_time</rdfs:label>
    <rdfs:comment>Last updated time of this resource.
A timestamp in RFC3339 UTC "Zulu" format, with nanosecond resolution and up to nine
fractional digits. Examples: "2014-10-02T15:01:23Z" and "2014-10-02T15:01:23.045123456Z".</rdfs:comment>
    <rdfs:domain rdf:resource="http://example.org/onto/class/google_vmwareengine_network_peering"/>
    <rdfs:range rdf:resource="http://www.w3.org/2001/XMLSchema#string"/>
  </owl:DatatypeProperty>
  <owl:DatatypeProperty rdf:about="http://example.org/onto/prop/google_vmwareengine_network_peering_vmware_engine_network">
    <rdfs:label>vmware_engine_network</rdfs:label>
    <rdfs:comment>The relative resource name of the VMware Engine network. Specify the name in the following form:
projects/{project}/locations/{location}/vmwareEngineNetworks/{vmwareEngineNetworkId} where {project}
can either be a project number or a project ID.</rdfs:comment>
    <rdfs:domain rdf:resource="http://example.org/onto/class/google_vmwareengine_network_peering"/>
    <rdfs:range rdf:resource="http://www.w3.org/2001/XMLSchema#string"/>
  </owl:DatatypeProperty>
  <owl:DatatypeProperty rdf:about="http://example.org/onto/prop/google_vmwareengine_network_peering_vmware_engine_network_canonical">
    <rdfs:label>vmware_engine_network_canonical</rdfs:label>
    <rdfs:comment>The canonical name of the VMware Engine network in the form:
projects/{project_number}/locations/{location}/vmwareEngineNetworks/{vmwareEngineNetworkId}</rdfs:comment>
    <rdfs:domain rdf:resource="http://example.org/onto/class/google_vmwareengine_network_peering"/>
    <rdfs:range rdf:resource="http://www.w3.org/2001/XMLSchema#string"/>
  </owl:DatatypeProperty>
  <owl:DatatypeProperty rdf:about="http://example.org/onto/prop/google_vmwareengine_network_peering_create">
    <rdfs:label>create</rdfs:label>
    <rdfs:domain rdf:resource="http://example.org/onto/class/google_vmwareengine_network_peering"/>
    <rdfs:range rdf:resource="http://www.w3.org/2001/XMLSchema#string"/>
  </owl:DatatypeProperty>
  <owl:DatatypeProperty rdf:about="http://example.org/onto/prop/google_vmwareengine_network_peering_delete">
    <rdfs:label>delete</rdfs:label>
    <rdfs:domain rdf:resource="http://example.org/onto/class/google_vmwareengine_network_peering"/>
    <rdfs:range rdf:resource="http://www.w3.org/2001/XMLSchema#string"/>
  </owl:DatatypeProperty>
  <owl:DatatypeProperty rdf:about="http://example.org/onto/prop/google_vmwareengine_network_peering_update">
    <rdfs:label>update</rdfs:label>
    <rdfs:domain rdf:resource="http://example.org/onto/class/google_vmwareengine_network_peering"/>
    <rdfs:range rdf:resource="http://www.w3.org/2001/XMLSchema#string"/>
  </owl:DatatypeProperty>
</rdf:RDF>
