<?xml version="1.0" encoding="UTF-8"?>
<rdf:RDF
  xmlns:rdf="http://www.w3.org/1999/02/22-rdf-syntax-ns#"
  xmlns:rdfs="http://www.w3.org/2000/01/rdf-schema#"
  xmlns:owl="http://www.w3.org/2002/07/owl#"
  xmlns:xsd="http://www.w3.org/2001/XMLSchema#"
  xml:base="http://example.org/onto/">
  <owl:Class rdf:about="http://example.org/onto/class/google_oracle_database_odb_network">
    <rdfs:label>google_oracle_database_odb_network</rdfs:label>
    <rdfs:comment>#
#     ***     AUTO GENERATED CODE    ***    Type: MMv1     ***
#
# ----------------------------------------------------------------------------
#
#     This code is generated by Magic Modules using the following:
#
#     Configuration: https:#github.com/GoogleCloudPlatform/magic-modules/tree/main/mmv1/products/oracledatabase/OdbNetwork.yaml
#     Template:      https:#github.com/GoogleCloudPlatform/magic-modules/tree/main/mmv1/templates/terraform/resource.html.markdown.tmpl
#
#     DO NOT EDIT this file directly. Any changes made to this file will be
#     overwritten during the next generation cycle.
#
# ----------------------------------------------------------------------------
subcategory: "Oracle Database"
description: |-
  An OdbNetwork resource which represents a private network providing connectivity between OracleDatabase resources and Google Cloud VPC network.
---</rdfs:comment>
  </owl:Class>
  <owl:DatatypeProperty rdf:about="http://example.org/onto/prop/google_oracle_database_odb_network_create_time">
    <rdfs:label>create_time</rdfs:label>
    <rdfs:comment>The date and time that the OdbNetwork was created.</rdfs:comment>
    <rdfs:domain rdf:resource="http://example.org/onto/class/google_oracle_database_odb_network"/>
    <rdfs:range rdf:resource="http://www.w3.org/2001/XMLSchema#string"/>
  </owl:DatatypeProperty>
  <owl:DatatypeProperty rdf:about="http://example.org/onto/prop/google_oracle_database_odb_network_deletion_protection">
    <rdfs:label>deletion_protection</rdfs:label>
    <rdfs:comment>Whether or not to allow Terraform to destroy the instance. Unless this field is set to false in Terraform state, a terraform destroy or terraform apply that would delete the instance will fail.</rdfs:comment>
    <rdfs:domain rdf:resource="http://example.org/onto/class/google_oracle_database_odb_network"/>
    <rdfs:range rdf:resource="http://www.w3.org/2001/XMLSchema#string"/>
  </owl:DatatypeProperty>
  <owl:DatatypeProperty rdf:about="http://example.org/onto/prop/google_oracle_database_odb_network_effective_labels">
    <rdfs:label>effective_labels</rdfs:label>
    <rdfs:comment>All of labels (key/value pairs) present on the resource in GCP, including the labels configured through Terraform, other clients and services.</rdfs:comment>
    <rdfs:domain rdf:resource="http://example.org/onto/class/google_oracle_database_odb_network"/>
    <rdfs:range rdf:resource="http://www.w3.org/2001/XMLSchema#string"/>
  </owl:DatatypeProperty>
  <owl:DatatypeProperty rdf:about="http://example.org/onto/prop/google_oracle_database_odb_network_entitlement_id">
    <rdfs:label>entitlement_id</rdfs:label>
    <rdfs:comment>The ID of the subscription entitlement associated with the OdbNetwork.</rdfs:comment>
    <rdfs:domain rdf:resource="http://example.org/onto/class/google_oracle_database_odb_network"/>
    <rdfs:range rdf:resource="http://www.w3.org/2001/XMLSchema#string"/>
  </owl:DatatypeProperty>
  <owl:DatatypeProperty rdf:about="http://example.org/onto/prop/google_oracle_database_odb_network_gcp_oracle_zone">
    <rdfs:label>gcp_oracle_zone</rdfs:label>
    <rdfs:comment>The GCP Oracle zone where OdbNetwork is hosted.
Example: us-east4-b-r2.
If not specified, the system will pick a zone based on availability.</rdfs:comment>
    <rdfs:domain rdf:resource="http://example.org/onto/class/google_oracle_database_odb_network"/>
    <rdfs:range rdf:resource="http://www.w3.org/2001/XMLSchema#string"/>
  </owl:DatatypeProperty>
  <owl:DatatypeProperty rdf:about="http://example.org/onto/prop/google_oracle_database_odb_network_id">
    <rdfs:label>id</rdfs:label>
    <rdfs:domain rdf:resource="http://example.org/onto/class/google_oracle_database_odb_network"/>
    <rdfs:range rdf:resource="http://www.w3.org/2001/XMLSchema#string"/>
  </owl:DatatypeProperty>
  <owl:DatatypeProperty rdf:about="http://example.org/onto/prop/google_oracle_database_odb_network_labels">
    <rdfs:label>labels</rdfs:label>
    <rdfs:comment>Labels or tags associated with the resource.

**Note**: This field is non-authoritative, and will only manage the labels present in your configuration.
Please refer to the field 'effective_labels' for all of the labels present on the resource.</rdfs:comment>
    <rdfs:domain rdf:resource="http://example.org/onto/class/google_oracle_database_odb_network"/>
    <rdfs:range rdf:resource="http://www.w3.org/2001/XMLSchema#string"/>
  </owl:DatatypeProperty>
  <owl:DatatypeProperty rdf:about="http://example.org/onto/prop/google_oracle_database_odb_network_location">
    <rdfs:label>location</rdfs:label>
    <rdfs:comment>Resource ID segment making up resource 'name'. It identifies the resource within its parent collection as described in https://google.aip.dev/122.</rdfs:comment>
    <rdfs:domain rdf:resource="http://example.org/onto/class/google_oracle_database_odb_network"/>
    <rdfs:range rdf:resource="http://www.w3.org/2001/XMLSchema#string"/>
  </owl:DatatypeProperty>
  <owl:DatatypeProperty rdf:about="http://example.org/onto/prop/google_oracle_database_odb_network_name">
    <rdfs:label>name</rdfs:label>
    <rdfs:comment>Identifier. The name of the OdbNetwork resource in the following format:
projects/{project}/locations/{region}/odbNetworks/{odb_network}</rdfs:comment>
    <rdfs:domain rdf:resource="http://example.org/onto/class/google_oracle_database_odb_network"/>
    <rdfs:range rdf:resource="http://www.w3.org/2001/XMLSchema#string"/>
  </owl:DatatypeProperty>
  <owl:DatatypeProperty rdf:about="http://example.org/onto/prop/google_oracle_database_odb_network_network">
    <rdfs:label>network</rdfs:label>
    <rdfs:comment>The name of the VPC network in the following format:
projects/{project}/global/networks/{network}</rdfs:comment>
    <rdfs:domain rdf:resource="http://example.org/onto/class/google_oracle_database_odb_network"/>
    <rdfs:range rdf:resource="http://www.w3.org/2001/XMLSchema#string"/>
  </owl:DatatypeProperty>
  <owl:DatatypeProperty rdf:about="http://example.org/onto/prop/google_oracle_database_odb_network_odb_network_id">
    <rdfs:label>odb_network_id</rdfs:label>
    <rdfs:comment>The ID of the OdbNetwork to create. This value is restricted
to (^[a-z]([a-z0-9-]{0,61}[a-z0-9])?$) and must be a maximum of 63
characters in length. The value must start with a letter and end with
a letter or a number.</rdfs:comment>
    <rdfs:domain rdf:resource="http://example.org/onto/class/google_oracle_database_odb_network"/>
    <rdfs:range rdf:resource="http://www.w3.org/2001/XMLSchema#string"/>
  </owl:DatatypeProperty>
  <owl:DatatypeProperty rdf:about="http://example.org/onto/prop/google_oracle_database_odb_network_project">
    <rdfs:label>project</rdfs:label>
    <rdfs:domain rdf:resource="http://example.org/onto/class/google_oracle_database_odb_network"/>
    <rdfs:range rdf:resource="http://www.w3.org/2001/XMLSchema#string"/>
  </owl:DatatypeProperty>
  <owl:DatatypeProperty rdf:about="http://example.org/onto/prop/google_oracle_database_odb_network_state">
    <rdfs:label>state</rdfs:label>
    <rdfs:comment>State of the ODB Network.
Possible values:
PROVISIONING
AVAILABLE
TERMINATING
FAILED</rdfs:comment>
    <rdfs:domain rdf:resource="http://example.org/onto/class/google_oracle_database_odb_network"/>
    <rdfs:range rdf:resource="http://www.w3.org/2001/XMLSchema#string"/>
  </owl:DatatypeProperty>
  <owl:DatatypeProperty rdf:about="http://example.org/onto/prop/google_oracle_database_odb_network_terraform_labels">
    <rdfs:label>terraform_labels</rdfs:label>
    <rdfs:comment>The combination of labels configured directly on the resource
 and default labels configured on the provider.</rdfs:comment>
    <rdfs:domain rdf:resource="http://example.org/onto/class/google_oracle_database_odb_network"/>
    <rdfs:range rdf:resource="http://www.w3.org/2001/XMLSchema#string"/>
  </owl:DatatypeProperty>
  <owl:DatatypeProperty rdf:about="http://example.org/onto/prop/google_oracle_database_odb_network_create">
    <rdfs:label>create</rdfs:label>
    <rdfs:domain rdf:resource="http://example.org/onto/class/google_oracle_database_odb_network"/>
    <rdfs:range rdf:resource="http://www.w3.org/2001/XMLSchema#string"/>
  </owl:DatatypeProperty>
  <owl:DatatypeProperty rdf:about="http://example.org/onto/prop/google_oracle_database_odb_network_delete">
    <rdfs:label>delete</rdfs:label>
    <rdfs:domain rdf:resource="http://example.org/onto/class/google_oracle_database_odb_network"/>
    <rdfs:range rdf:resource="http://www.w3.org/2001/XMLSchema#string"/>
  </owl:DatatypeProperty>
  <owl:DatatypeProperty rdf:about="http://example.org/onto/prop/google_oracle_database_odb_network_update">
    <rdfs:label>update</rdfs:label>
    <rdfs:domain rdf:resource="http://example.org/onto/class/google_oracle_database_odb_network"/>
    <rdfs:range rdf:resource="http://www.w3.org/2001/XMLSchema#string"/>
  </owl:DatatypeProperty>
</rdf:RDF>
