<?xml version="1.0" encoding="UTF-8"?>
<rdf:RDF
  xmlns:rdf="http://www.w3.org/1999/02/22-rdf-syntax-ns#"
  xmlns:rdfs="http://www.w3.org/2000/01/rdf-schema#"
  xmlns:owl="http://www.w3.org/2002/07/owl#"
  xmlns:xsd="http://www.w3.org/2001/XMLSchema#"
  xml:base="http://example.org/onto/">
  <owl:Class rdf:about="http://example.org/onto/class/google_notebooks_instance">
    <rdfs:label>google_notebooks_instance</rdfs:label>
    <rdfs:comment>#
#     ***     AUTO GENERATED CODE    ***    Type: MMv1     ***
#
# ----------------------------------------------------------------------------
#
#     This code is generated by Magic Modules using the following:
#
#     Configuration: https:#github.com/GoogleCloudPlatform/magic-modules/tree/main/mmv1/products/notebooks/Instance.yaml
#     Template:      https:#github.com/GoogleCloudPlatform/magic-modules/tree/main/mmv1/templates/terraform/resource.html.markdown.tmpl
#
#     DO NOT EDIT this file directly. Any changes made to this file will be
#     overwritten during the next generation cycle.
#
# ----------------------------------------------------------------------------
subcategory: "Cloud AI Notebooks"
description: |-
  A Cloud AI Platform Notebook instance.
---</rdfs:comment>
  </owl:Class>
  <owl:DatatypeProperty rdf:about="http://example.org/onto/prop/google_notebooks_instance_boot_disk_size_gb">
    <rdfs:label>boot_disk_size_gb</rdfs:label>
    <rdfs:comment>The size of the boot disk in GB attached to this instance,
up to a maximum of 64000 GB (64 TB). The minimum recommended value is 100 GB.
If not specified, this defaults to 100.</rdfs:comment>
    <rdfs:domain rdf:resource="http://example.org/onto/class/google_notebooks_instance"/>
    <rdfs:range rdf:resource="http://www.w3.org/2001/XMLSchema#string"/>
  </owl:DatatypeProperty>
  <owl:DatatypeProperty rdf:about="http://example.org/onto/prop/google_notebooks_instance_boot_disk_type">
    <rdfs:label>boot_disk_type</rdfs:label>
    <rdfs:comment>Possible disk types for notebook instances. Possible values: ["DISK_TYPE_UNSPECIFIED", "PD_STANDARD", "PD_SSD", "PD_BALANCED", "PD_EXTREME"]</rdfs:comment>
    <rdfs:domain rdf:resource="http://example.org/onto/class/google_notebooks_instance"/>
    <rdfs:range rdf:resource="http://www.w3.org/2001/XMLSchema#string"/>
  </owl:DatatypeProperty>
  <owl:DatatypeProperty rdf:about="http://example.org/onto/prop/google_notebooks_instance_create_time">
    <rdfs:label>create_time</rdfs:label>
    <rdfs:comment>Instance creation time</rdfs:comment>
    <rdfs:domain rdf:resource="http://example.org/onto/class/google_notebooks_instance"/>
    <rdfs:range rdf:resource="http://www.w3.org/2001/XMLSchema#string"/>
  </owl:DatatypeProperty>
  <owl:DatatypeProperty rdf:about="http://example.org/onto/prop/google_notebooks_instance_custom_gpu_driver_path">
    <rdfs:label>custom_gpu_driver_path</rdfs:label>
    <rdfs:comment>Specify a custom Cloud Storage path where the GPU driver is stored.
If not specified, we'll automatically choose from official GPU drivers.</rdfs:comment>
    <rdfs:domain rdf:resource="http://example.org/onto/class/google_notebooks_instance"/>
    <rdfs:range rdf:resource="http://www.w3.org/2001/XMLSchema#string"/>
  </owl:DatatypeProperty>
  <owl:DatatypeProperty rdf:about="http://example.org/onto/prop/google_notebooks_instance_data_disk_size_gb">
    <rdfs:label>data_disk_size_gb</rdfs:label>
    <rdfs:comment>The size of the data disk in GB attached to this instance,
up to a maximum of 64000 GB (64 TB).
You can choose the size of the data disk based on how big your notebooks and data are.
If not specified, this defaults to 100.</rdfs:comment>
    <rdfs:domain rdf:resource="http://example.org/onto/class/google_notebooks_instance"/>
    <rdfs:range rdf:resource="http://www.w3.org/2001/XMLSchema#string"/>
  </owl:DatatypeProperty>
  <owl:DatatypeProperty rdf:about="http://example.org/onto/prop/google_notebooks_instance_data_disk_type">
    <rdfs:label>data_disk_type</rdfs:label>
    <rdfs:comment>Possible disk types for notebook instances. Possible values: ["DISK_TYPE_UNSPECIFIED", "PD_STANDARD", "PD_SSD", "PD_BALANCED", "PD_EXTREME"]</rdfs:comment>
    <rdfs:domain rdf:resource="http://example.org/onto/class/google_notebooks_instance"/>
    <rdfs:range rdf:resource="http://www.w3.org/2001/XMLSchema#string"/>
  </owl:DatatypeProperty>
  <owl:DatatypeProperty rdf:about="http://example.org/onto/prop/google_notebooks_instance_desired_state">
    <rdfs:label>desired_state</rdfs:label>
    <rdfs:comment>Desired state of the Notebook Instance. Set this field to 'ACTIVE' to start the Instance, and 'STOPPED' to stop the Instance.</rdfs:comment>
    <rdfs:domain rdf:resource="http://example.org/onto/class/google_notebooks_instance"/>
    <rdfs:range rdf:resource="http://www.w3.org/2001/XMLSchema#string"/>
  </owl:DatatypeProperty>
  <owl:DatatypeProperty rdf:about="http://example.org/onto/prop/google_notebooks_instance_disk_encryption">
    <rdfs:label>disk_encryption</rdfs:label>
    <rdfs:comment>Disk encryption method used on the boot and data disks, defaults to GMEK. Possible values: ["DISK_ENCRYPTION_UNSPECIFIED", "GMEK", "CMEK"]</rdfs:comment>
    <rdfs:domain rdf:resource="http://example.org/onto/class/google_notebooks_instance"/>
    <rdfs:range rdf:resource="http://www.w3.org/2001/XMLSchema#string"/>
  </owl:DatatypeProperty>
  <owl:DatatypeProperty rdf:about="http://example.org/onto/prop/google_notebooks_instance_effective_labels">
    <rdfs:label>effective_labels</rdfs:label>
    <rdfs:comment>All of labels (key/value pairs) present on the resource in GCP, including the labels configured through Terraform, other clients and services.</rdfs:comment>
    <rdfs:domain rdf:resource="http://example.org/onto/class/google_notebooks_instance"/>
    <rdfs:range rdf:resource="http://www.w3.org/2001/XMLSchema#string"/>
  </owl:DatatypeProperty>
  <owl:DatatypeProperty rdf:about="http://example.org/onto/prop/google_notebooks_instance_id">
    <rdfs:label>id</rdfs:label>
    <rdfs:domain rdf:resource="http://example.org/onto/class/google_notebooks_instance"/>
    <rdfs:range rdf:resource="http://www.w3.org/2001/XMLSchema#string"/>
  </owl:DatatypeProperty>
  <owl:DatatypeProperty rdf:about="http://example.org/onto/prop/google_notebooks_instance_install_gpu_driver">
    <rdfs:label>install_gpu_driver</rdfs:label>
    <rdfs:comment>Whether the end user authorizes Google Cloud to install GPU driver
on this instance. If this field is empty or set to false, the GPU driver
won't be installed. Only applicable to instances with GPUs.</rdfs:comment>
    <rdfs:domain rdf:resource="http://example.org/onto/class/google_notebooks_instance"/>
    <rdfs:range rdf:resource="http://www.w3.org/2001/XMLSchema#string"/>
  </owl:DatatypeProperty>
  <owl:DatatypeProperty rdf:about="http://example.org/onto/prop/google_notebooks_instance_instance_owners">
    <rdfs:label>instance_owners</rdfs:label>
    <rdfs:comment>The list of owners of this instance after creation.
Format: alias@example.com.
Currently supports one owner only.
If not specified, all of the service account users of
your VM instance's service account can use the instance.</rdfs:comment>
    <rdfs:domain rdf:resource="http://example.org/onto/class/google_notebooks_instance"/>
    <rdfs:range rdf:resource="http://www.w3.org/2001/XMLSchema#string"/>
  </owl:DatatypeProperty>
  <owl:DatatypeProperty rdf:about="http://example.org/onto/prop/google_notebooks_instance_kms_key">
    <rdfs:label>kms_key</rdfs:label>
    <rdfs:comment>The KMS key used to encrypt the disks, only applicable if diskEncryption is CMEK.
Format: projects/{project_id}/locations/{location}/keyRings/{key_ring_id}/cryptoKeys/{key_id}</rdfs:comment>
    <rdfs:domain rdf:resource="http://example.org/onto/class/google_notebooks_instance"/>
    <rdfs:range rdf:resource="http://www.w3.org/2001/XMLSchema#string"/>
  </owl:DatatypeProperty>
  <owl:DatatypeProperty rdf:about="http://example.org/onto/prop/google_notebooks_instance_labels">
    <rdfs:label>labels</rdfs:label>
    <rdfs:comment>Labels to apply to this instance. These can be later modified by the setLabels method.
An object containing a list of "key": value pairs. Example: { "name": "wrench", "mass": "1.3kg", "count": "3" }.


**Note**: This field is non-authoritative, and will only manage the labels present in your configuration.
Please refer to the field 'effective_labels' for all of the labels present on the resource.</rdfs:comment>
    <rdfs:domain rdf:resource="http://example.org/onto/class/google_notebooks_instance"/>
    <rdfs:range rdf:resource="http://www.w3.org/2001/XMLSchema#string"/>
  </owl:DatatypeProperty>
  <owl:DatatypeProperty rdf:about="http://example.org/onto/prop/google_notebooks_instance_location">
    <rdfs:label>location</rdfs:label>
    <rdfs:comment>A reference to the zone where the machine resides.</rdfs:comment>
    <rdfs:domain rdf:resource="http://example.org/onto/class/google_notebooks_instance"/>
    <rdfs:range rdf:resource="http://www.w3.org/2001/XMLSchema#string"/>
  </owl:DatatypeProperty>
  <owl:DatatypeProperty rdf:about="http://example.org/onto/prop/google_notebooks_instance_machine_type">
    <rdfs:label>machine_type</rdfs:label>
    <rdfs:comment>A reference to a machine type which defines VM kind.</rdfs:comment>
    <rdfs:domain rdf:resource="http://example.org/onto/class/google_notebooks_instance"/>
    <rdfs:range rdf:resource="http://www.w3.org/2001/XMLSchema#string"/>
  </owl:DatatypeProperty>
  <owl:DatatypeProperty rdf:about="http://example.org/onto/prop/google_notebooks_instance_metadata">
    <rdfs:label>metadata</rdfs:label>
    <rdfs:comment>Custom metadata to apply to this instance.
An object containing a list of "key": value pairs. Example: { "name": "wrench", "mass": "1.3kg", "count": "3" }.</rdfs:comment>
    <rdfs:domain rdf:resource="http://example.org/onto/class/google_notebooks_instance"/>
    <rdfs:range rdf:resource="http://www.w3.org/2001/XMLSchema#string"/>
  </owl:DatatypeProperty>
  <owl:DatatypeProperty rdf:about="http://example.org/onto/prop/google_notebooks_instance_name">
    <rdfs:label>name</rdfs:label>
    <rdfs:comment>The name specified for the Notebook instance.</rdfs:comment>
    <rdfs:domain rdf:resource="http://example.org/onto/class/google_notebooks_instance"/>
    <rdfs:range rdf:resource="http://www.w3.org/2001/XMLSchema#string"/>
  </owl:DatatypeProperty>
  <owl:DatatypeProperty rdf:about="http://example.org/onto/prop/google_notebooks_instance_network">
    <rdfs:label>network</rdfs:label>
    <rdfs:comment>The name of the VPC that this instance is in.
Format: projects/{project_id}/global/networks/{network_id}</rdfs:comment>
    <rdfs:domain rdf:resource="http://example.org/onto/class/google_notebooks_instance"/>
    <rdfs:range rdf:resource="http://www.w3.org/2001/XMLSchema#string"/>
  </owl:DatatypeProperty>
  <owl:DatatypeProperty rdf:about="http://example.org/onto/prop/google_notebooks_instance_nic_type">
    <rdfs:label>nic_type</rdfs:label>
    <rdfs:comment>The type of vNIC driver. Possible values: ["UNSPECIFIED_NIC_TYPE", "VIRTIO_NET", "GVNIC"]</rdfs:comment>
    <rdfs:domain rdf:resource="http://example.org/onto/class/google_notebooks_instance"/>
    <rdfs:range rdf:resource="http://www.w3.org/2001/XMLSchema#string"/>
  </owl:DatatypeProperty>
  <owl:DatatypeProperty rdf:about="http://example.org/onto/prop/google_notebooks_instance_no_proxy_access">
    <rdfs:label>no_proxy_access</rdfs:label>
    <rdfs:comment>The notebook instance will not register with the proxy..</rdfs:comment>
    <rdfs:domain rdf:resource="http://example.org/onto/class/google_notebooks_instance"/>
    <rdfs:range rdf:resource="http://www.w3.org/2001/XMLSchema#string"/>
  </owl:DatatypeProperty>
  <owl:DatatypeProperty rdf:about="http://example.org/onto/prop/google_notebooks_instance_no_public_ip">
    <rdfs:label>no_public_ip</rdfs:label>
    <rdfs:comment>No public IP will be assigned to this instance.</rdfs:comment>
    <rdfs:domain rdf:resource="http://example.org/onto/class/google_notebooks_instance"/>
    <rdfs:range rdf:resource="http://www.w3.org/2001/XMLSchema#string"/>
  </owl:DatatypeProperty>
  <owl:DatatypeProperty rdf:about="http://example.org/onto/prop/google_notebooks_instance_no_remove_data_disk">
    <rdfs:label>no_remove_data_disk</rdfs:label>
    <rdfs:comment>If true, the data disk will not be auto deleted when deleting the instance.</rdfs:comment>
    <rdfs:domain rdf:resource="http://example.org/onto/class/google_notebooks_instance"/>
    <rdfs:range rdf:resource="http://www.w3.org/2001/XMLSchema#string"/>
  </owl:DatatypeProperty>
  <owl:DatatypeProperty rdf:about="http://example.org/onto/prop/google_notebooks_instance_post_startup_script">
    <rdfs:label>post_startup_script</rdfs:label>
    <rdfs:comment>Path to a Bash script that automatically runs after a
notebook instance fully boots up. The path must be a URL
or Cloud Storage path (gs://path-to-file/file-name).</rdfs:comment>
    <rdfs:domain rdf:resource="http://example.org/onto/class/google_notebooks_instance"/>
    <rdfs:range rdf:resource="http://www.w3.org/2001/XMLSchema#string"/>
  </owl:DatatypeProperty>
  <owl:DatatypeProperty rdf:about="http://example.org/onto/prop/google_notebooks_instance_project">
    <rdfs:label>project</rdfs:label>
    <rdfs:domain rdf:resource="http://example.org/onto/class/google_notebooks_instance"/>
    <rdfs:range rdf:resource="http://www.w3.org/2001/XMLSchema#string"/>
  </owl:DatatypeProperty>
  <owl:DatatypeProperty rdf:about="http://example.org/onto/prop/google_notebooks_instance_proxy_uri">
    <rdfs:label>proxy_uri</rdfs:label>
    <rdfs:comment>The proxy endpoint that is used to access the Jupyter notebook.
Only returned when the resource is in a 'PROVISIONED' state. If
needed you can utilize 'terraform apply -refresh-only' to await
the population of this value.</rdfs:comment>
    <rdfs:domain rdf:resource="http://example.org/onto/class/google_notebooks_instance"/>
    <rdfs:range rdf:resource="http://www.w3.org/2001/XMLSchema#string"/>
  </owl:DatatypeProperty>
  <owl:DatatypeProperty rdf:about="http://example.org/onto/prop/google_notebooks_instance_service_account">
    <rdfs:label>service_account</rdfs:label>
    <rdfs:comment>The service account on this instance, giving access to other
Google Cloud services. You can use any service account within
the same project, but you must have the service account user
permission to use the instance. If not specified,
the Compute Engine default service account is used.</rdfs:comment>
    <rdfs:domain rdf:resource="http://example.org/onto/class/google_notebooks_instance"/>
    <rdfs:range rdf:resource="http://www.w3.org/2001/XMLSchema#string"/>
  </owl:DatatypeProperty>
  <owl:DatatypeProperty rdf:about="http://example.org/onto/prop/google_notebooks_instance_service_account_scopes">
    <rdfs:label>service_account_scopes</rdfs:label>
    <rdfs:comment>Optional. The URIs of service account scopes to be included in Compute Engine instances.
If not specified, the following scopes are defined:
- https://www.googleapis.com/auth/cloud-platform
- https://www.googleapis.com/auth/userinfo.email</rdfs:comment>
    <rdfs:domain rdf:resource="http://example.org/onto/class/google_notebooks_instance"/>
    <rdfs:range rdf:resource="http://www.w3.org/2001/XMLSchema#string"/>
  </owl:DatatypeProperty>
  <owl:DatatypeProperty rdf:about="http://example.org/onto/prop/google_notebooks_instance_state">
    <rdfs:label>state</rdfs:label>
    <rdfs:comment>The state of this instance.</rdfs:comment>
    <rdfs:domain rdf:resource="http://example.org/onto/class/google_notebooks_instance"/>
    <rdfs:range rdf:resource="http://www.w3.org/2001/XMLSchema#string"/>
  </owl:DatatypeProperty>
  <owl:DatatypeProperty rdf:about="http://example.org/onto/prop/google_notebooks_instance_subnet">
    <rdfs:label>subnet</rdfs:label>
    <rdfs:comment>The name of the subnet that this instance is in.
Format: projects/{project_id}/regions/{region}/subnetworks/{subnetwork_id}</rdfs:comment>
    <rdfs:domain rdf:resource="http://example.org/onto/class/google_notebooks_instance"/>
    <rdfs:range rdf:resource="http://www.w3.org/2001/XMLSchema#string"/>
  </owl:DatatypeProperty>
  <owl:DatatypeProperty rdf:about="http://example.org/onto/prop/google_notebooks_instance_tags">
    <rdfs:label>tags</rdfs:label>
    <rdfs:comment>The Compute Engine tags to add to instance.</rdfs:comment>
    <rdfs:domain rdf:resource="http://example.org/onto/class/google_notebooks_instance"/>
    <rdfs:range rdf:resource="http://www.w3.org/2001/XMLSchema#string"/>
  </owl:DatatypeProperty>
  <owl:DatatypeProperty rdf:about="http://example.org/onto/prop/google_notebooks_instance_terraform_labels">
    <rdfs:label>terraform_labels</rdfs:label>
    <rdfs:comment>The combination of labels configured directly on the resource
 and default labels configured on the provider.</rdfs:comment>
    <rdfs:domain rdf:resource="http://example.org/onto/class/google_notebooks_instance"/>
    <rdfs:range rdf:resource="http://www.w3.org/2001/XMLSchema#string"/>
  </owl:DatatypeProperty>
  <owl:DatatypeProperty rdf:about="http://example.org/onto/prop/google_notebooks_instance_update_time">
    <rdfs:label>update_time</rdfs:label>
    <rdfs:comment>Instance update time.</rdfs:comment>
    <rdfs:domain rdf:resource="http://example.org/onto/class/google_notebooks_instance"/>
    <rdfs:range rdf:resource="http://www.w3.org/2001/XMLSchema#string"/>
  </owl:DatatypeProperty>
  <owl:DatatypeProperty rdf:about="http://example.org/onto/prop/google_notebooks_instance_core_count">
    <rdfs:label>core_count</rdfs:label>
    <rdfs:comment>Count of cores of this accelerator.</rdfs:comment>
    <rdfs:domain rdf:resource="http://example.org/onto/class/google_notebooks_instance"/>
    <rdfs:range rdf:resource="http://www.w3.org/2001/XMLSchema#string"/>
  </owl:DatatypeProperty>
  <owl:DatatypeProperty rdf:about="http://example.org/onto/prop/google_notebooks_instance_type">
    <rdfs:label>type</rdfs:label>
    <rdfs:comment>Type of this accelerator. Possible values: ["ACCELERATOR_TYPE_UNSPECIFIED", "NVIDIA_TESLA_K80", "NVIDIA_TESLA_P100", "NVIDIA_TESLA_V100", "NVIDIA_TESLA_P4", "NVIDIA_TESLA_T4", "NVIDIA_TESLA_T4_VWS", "NVIDIA_TESLA_P100_VWS", "NVIDIA_TESLA_P4_VWS", "NVIDIA_TESLA_A100", "TPU_V2", "TPU_V3"]</rdfs:comment>
    <rdfs:domain rdf:resource="http://example.org/onto/class/google_notebooks_instance"/>
    <rdfs:range rdf:resource="http://www.w3.org/2001/XMLSchema#string"/>
  </owl:DatatypeProperty>
  <owl:DatatypeProperty rdf:about="http://example.org/onto/prop/google_notebooks_instance_repository">
    <rdfs:label>repository</rdfs:label>
    <rdfs:comment>The path to the container image repository.
For example: gcr.io/{project_id}/{imageName}</rdfs:comment>
    <rdfs:domain rdf:resource="http://example.org/onto/class/google_notebooks_instance"/>
    <rdfs:range rdf:resource="http://www.w3.org/2001/XMLSchema#string"/>
  </owl:DatatypeProperty>
  <owl:DatatypeProperty rdf:about="http://example.org/onto/prop/google_notebooks_instance_tag">
    <rdfs:label>tag</rdfs:label>
    <rdfs:comment>The tag of the container image. If not specified, this defaults to the latest tag.</rdfs:comment>
    <rdfs:domain rdf:resource="http://example.org/onto/class/google_notebooks_instance"/>
    <rdfs:range rdf:resource="http://www.w3.org/2001/XMLSchema#string"/>
  </owl:DatatypeProperty>
  <owl:DatatypeProperty rdf:about="http://example.org/onto/prop/google_notebooks_instance_consume_reservation_type">
    <rdfs:label>consume_reservation_type</rdfs:label>
    <rdfs:comment>The type of Compute Reservation. Possible values: ["NO_RESERVATION", "ANY_RESERVATION", "SPECIFIC_RESERVATION"]</rdfs:comment>
    <rdfs:domain rdf:resource="http://example.org/onto/class/google_notebooks_instance"/>
    <rdfs:range rdf:resource="http://www.w3.org/2001/XMLSchema#string"/>
  </owl:DatatypeProperty>
  <owl:DatatypeProperty rdf:about="http://example.org/onto/prop/google_notebooks_instance_key">
    <rdfs:label>key</rdfs:label>
    <rdfs:comment>Corresponds to the label key of reservation resource.</rdfs:comment>
    <rdfs:domain rdf:resource="http://example.org/onto/class/google_notebooks_instance"/>
    <rdfs:range rdf:resource="http://www.w3.org/2001/XMLSchema#string"/>
  </owl:DatatypeProperty>
  <owl:DatatypeProperty rdf:about="http://example.org/onto/prop/google_notebooks_instance_values">
    <rdfs:label>values</rdfs:label>
    <rdfs:comment>Corresponds to the label values of reservation resource.</rdfs:comment>
    <rdfs:domain rdf:resource="http://example.org/onto/class/google_notebooks_instance"/>
    <rdfs:range rdf:resource="http://www.w3.org/2001/XMLSchema#string"/>
  </owl:DatatypeProperty>
  <owl:DatatypeProperty rdf:about="http://example.org/onto/prop/google_notebooks_instance_enable_integrity_monitoring">
    <rdfs:label>enable_integrity_monitoring</rdfs:label>
    <rdfs:comment>Defines whether the instance has integrity monitoring enabled. Enables monitoring and attestation of the
boot integrity of the instance. The attestation is performed against the integrity policy baseline.
This baseline is initially derived from the implicitly trusted boot image when the instance is created.
Enabled by default.</rdfs:comment>
    <rdfs:domain rdf:resource="http://example.org/onto/class/google_notebooks_instance"/>
    <rdfs:range rdf:resource="http://www.w3.org/2001/XMLSchema#string"/>
  </owl:DatatypeProperty>
  <owl:DatatypeProperty rdf:about="http://example.org/onto/prop/google_notebooks_instance_enable_secure_boot">
    <rdfs:label>enable_secure_boot</rdfs:label>
    <rdfs:comment>Defines whether the instance has Secure Boot enabled. Secure Boot helps ensure that the system only runs
authentic software by verifying the digital signature of all boot components, and halting the boot process
if signature verification fails.
Disabled by default.</rdfs:comment>
    <rdfs:domain rdf:resource="http://example.org/onto/class/google_notebooks_instance"/>
    <rdfs:range rdf:resource="http://www.w3.org/2001/XMLSchema#string"/>
  </owl:DatatypeProperty>
  <owl:DatatypeProperty rdf:about="http://example.org/onto/prop/google_notebooks_instance_enable_vtpm">
    <rdfs:label>enable_vtpm</rdfs:label>
    <rdfs:comment>Defines whether the instance has the vTPM enabled.
Enabled by default.</rdfs:comment>
    <rdfs:domain rdf:resource="http://example.org/onto/class/google_notebooks_instance"/>
    <rdfs:range rdf:resource="http://www.w3.org/2001/XMLSchema#string"/>
  </owl:DatatypeProperty>
  <owl:DatatypeProperty rdf:about="http://example.org/onto/prop/google_notebooks_instance_create">
    <rdfs:label>create</rdfs:label>
    <rdfs:domain rdf:resource="http://example.org/onto/class/google_notebooks_instance"/>
    <rdfs:range rdf:resource="http://www.w3.org/2001/XMLSchema#string"/>
  </owl:DatatypeProperty>
  <owl:DatatypeProperty rdf:about="http://example.org/onto/prop/google_notebooks_instance_delete">
    <rdfs:label>delete</rdfs:label>
    <rdfs:domain rdf:resource="http://example.org/onto/class/google_notebooks_instance"/>
    <rdfs:range rdf:resource="http://www.w3.org/2001/XMLSchema#string"/>
  </owl:DatatypeProperty>
  <owl:DatatypeProperty rdf:about="http://example.org/onto/prop/google_notebooks_instance_update">
    <rdfs:label>update</rdfs:label>
    <rdfs:domain rdf:resource="http://example.org/onto/class/google_notebooks_instance"/>
    <rdfs:range rdf:resource="http://www.w3.org/2001/XMLSchema#string"/>
  </owl:DatatypeProperty>
  <owl:DatatypeProperty rdf:about="http://example.org/onto/prop/google_notebooks_instance_image_family">
    <rdfs:label>image_family</rdfs:label>
    <rdfs:comment>Use this VM image family to find the image; the newest image in this family will be used.</rdfs:comment>
    <rdfs:domain rdf:resource="http://example.org/onto/class/google_notebooks_instance"/>
    <rdfs:range rdf:resource="http://www.w3.org/2001/XMLSchema#string"/>
  </owl:DatatypeProperty>
  <owl:DatatypeProperty rdf:about="http://example.org/onto/prop/google_notebooks_instance_image_name">
    <rdfs:label>image_name</rdfs:label>
    <rdfs:comment>Use VM image name to find the image.</rdfs:comment>
    <rdfs:domain rdf:resource="http://example.org/onto/class/google_notebooks_instance"/>
    <rdfs:range rdf:resource="http://www.w3.org/2001/XMLSchema#string"/>
  </owl:DatatypeProperty>
  <owl:DatatypeProperty rdf:about="http://example.org/onto/prop/google_notebooks_instance_project">
    <rdfs:label>project</rdfs:label>
    <rdfs:comment>The name of the Google Cloud project that this VM image belongs to.
Format: projects/{project_id}</rdfs:comment>
    <rdfs:domain rdf:resource="http://example.org/onto/class/google_notebooks_instance"/>
    <rdfs:range rdf:resource="http://www.w3.org/2001/XMLSchema#string"/>
  </owl:DatatypeProperty>
</rdf:RDF>
