<?xml version="1.0" encoding="UTF-8"?>
<rdf:RDF
  xmlns:rdf="http://www.w3.org/1999/02/22-rdf-syntax-ns#"
  xmlns:rdfs="http://www.w3.org/2000/01/rdf-schema#"
  xmlns:owl="http://www.w3.org/2002/07/owl#"
  xmlns:xsd="http://www.w3.org/2001/XMLSchema#"
  xml:base="http://example.org/onto/">
  <owl:Class rdf:about="http://example.org/onto/class/google_network_connectivity_group">
    <rdfs:label>google_network_connectivity_group</rdfs:label>
    <rdfs:comment>#
#     ***     AUTO GENERATED CODE    ***    Type: MMv1     ***
#
# ----------------------------------------------------------------------------
#
#     This code is generated by Magic Modules using the following:
#
#     Configuration: https:#github.com/GoogleCloudPlatform/magic-modules/tree/main/mmv1/products/networkconnectivity/Group.yaml
#     Template:      https:#github.com/GoogleCloudPlatform/magic-modules/tree/main/mmv1/templates/terraform/resource.html.markdown.tmpl
#
#     DO NOT EDIT this file directly. Any changes made to this file will be
#     overwritten during the next generation cycle.
#
# ----------------------------------------------------------------------------
subcategory: "Network Connectivity"
description: |-
  The NetworkConnectivity Group resource
---</rdfs:comment>
  </owl:Class>
  <owl:DatatypeProperty rdf:about="http://example.org/onto/prop/google_network_connectivity_group_create_time">
    <rdfs:label>create_time</rdfs:label>
    <rdfs:comment>Output only. The time the hub was created.</rdfs:comment>
    <rdfs:domain rdf:resource="http://example.org/onto/class/google_network_connectivity_group"/>
    <rdfs:range rdf:resource="http://www.w3.org/2001/XMLSchema#string"/>
  </owl:DatatypeProperty>
  <owl:DatatypeProperty rdf:about="http://example.org/onto/prop/google_network_connectivity_group_description">
    <rdfs:label>description</rdfs:label>
    <rdfs:comment>An optional description of the group.</rdfs:comment>
    <rdfs:domain rdf:resource="http://example.org/onto/class/google_network_connectivity_group"/>
    <rdfs:range rdf:resource="http://www.w3.org/2001/XMLSchema#string"/>
  </owl:DatatypeProperty>
  <owl:DatatypeProperty rdf:about="http://example.org/onto/prop/google_network_connectivity_group_effective_labels">
    <rdfs:label>effective_labels</rdfs:label>
    <rdfs:comment>All of labels (key/value pairs) present on the resource in GCP, including the labels configured through Terraform, other clients and services.</rdfs:comment>
    <rdfs:domain rdf:resource="http://example.org/onto/class/google_network_connectivity_group"/>
    <rdfs:range rdf:resource="http://www.w3.org/2001/XMLSchema#string"/>
  </owl:DatatypeProperty>
  <owl:DatatypeProperty rdf:about="http://example.org/onto/prop/google_network_connectivity_group_hub">
    <rdfs:label>hub</rdfs:label>
    <rdfs:comment>The name of the hub. Hub names must be unique. They use the following form: projects/{projectNumber}/locations/global/hubs/{hubId}</rdfs:comment>
    <rdfs:domain rdf:resource="http://example.org/onto/class/google_network_connectivity_group"/>
    <rdfs:range rdf:resource="http://www.w3.org/2001/XMLSchema#string"/>
  </owl:DatatypeProperty>
  <owl:DatatypeProperty rdf:about="http://example.org/onto/prop/google_network_connectivity_group_id">
    <rdfs:label>id</rdfs:label>
    <rdfs:domain rdf:resource="http://example.org/onto/class/google_network_connectivity_group"/>
    <rdfs:range rdf:resource="http://www.w3.org/2001/XMLSchema#string"/>
  </owl:DatatypeProperty>
  <owl:DatatypeProperty rdf:about="http://example.org/onto/prop/google_network_connectivity_group_labels">
    <rdfs:label>labels</rdfs:label>
    <rdfs:comment>Optional labels in key:value format. For more information about labels, see [Requirements for labels](https://cloud.google.com/resource-manager/docs/creating-managing-labels#requirements).

**Note**: This field is non-authoritative, and will only manage the labels present in your configuration.
Please refer to the field 'effective_labels' for all of the labels present on the resource.</rdfs:comment>
    <rdfs:domain rdf:resource="http://example.org/onto/class/google_network_connectivity_group"/>
    <rdfs:range rdf:resource="http://www.w3.org/2001/XMLSchema#string"/>
  </owl:DatatypeProperty>
  <owl:DatatypeProperty rdf:about="http://example.org/onto/prop/google_network_connectivity_group_name">
    <rdfs:label>name</rdfs:label>
    <rdfs:comment>The name of the group. Group names must be unique. Possible values: ["default", "center", "edge"]</rdfs:comment>
    <rdfs:domain rdf:resource="http://example.org/onto/class/google_network_connectivity_group"/>
    <rdfs:range rdf:resource="http://www.w3.org/2001/XMLSchema#string"/>
  </owl:DatatypeProperty>
  <owl:DatatypeProperty rdf:about="http://example.org/onto/prop/google_network_connectivity_group_project">
    <rdfs:label>project</rdfs:label>
    <rdfs:domain rdf:resource="http://example.org/onto/class/google_network_connectivity_group"/>
    <rdfs:range rdf:resource="http://www.w3.org/2001/XMLSchema#string"/>
  </owl:DatatypeProperty>
  <owl:DatatypeProperty rdf:about="http://example.org/onto/prop/google_network_connectivity_group_route_table">
    <rdfs:label>route_table</rdfs:label>
    <rdfs:comment>Output only. The name of the route table that corresponds to this group. They use the following form: 'projects/{projectNumber}/locations/global/hubs/{hubId}/routeTables/{route_table_id}'</rdfs:comment>
    <rdfs:domain rdf:resource="http://example.org/onto/class/google_network_connectivity_group"/>
    <rdfs:range rdf:resource="http://www.w3.org/2001/XMLSchema#string"/>
  </owl:DatatypeProperty>
  <owl:DatatypeProperty rdf:about="http://example.org/onto/prop/google_network_connectivity_group_state">
    <rdfs:label>state</rdfs:label>
    <rdfs:comment>Output only. The current lifecycle state of this hub.</rdfs:comment>
    <rdfs:domain rdf:resource="http://example.org/onto/class/google_network_connectivity_group"/>
    <rdfs:range rdf:resource="http://www.w3.org/2001/XMLSchema#string"/>
  </owl:DatatypeProperty>
  <owl:DatatypeProperty rdf:about="http://example.org/onto/prop/google_network_connectivity_group_terraform_labels">
    <rdfs:label>terraform_labels</rdfs:label>
    <rdfs:comment>The combination of labels configured directly on the resource
 and default labels configured on the provider.</rdfs:comment>
    <rdfs:domain rdf:resource="http://example.org/onto/class/google_network_connectivity_group"/>
    <rdfs:range rdf:resource="http://www.w3.org/2001/XMLSchema#string"/>
  </owl:DatatypeProperty>
  <owl:DatatypeProperty rdf:about="http://example.org/onto/prop/google_network_connectivity_group_uid">
    <rdfs:label>uid</rdfs:label>
    <rdfs:comment>Output only. The Google-generated UUID for the group. This value is unique across all group resources. If a group is deleted and another with the same name is created, the new route table is assigned a different uniqueId.</rdfs:comment>
    <rdfs:domain rdf:resource="http://example.org/onto/class/google_network_connectivity_group"/>
    <rdfs:range rdf:resource="http://www.w3.org/2001/XMLSchema#string"/>
  </owl:DatatypeProperty>
  <owl:DatatypeProperty rdf:about="http://example.org/onto/prop/google_network_connectivity_group_update_time">
    <rdfs:label>update_time</rdfs:label>
    <rdfs:comment>Output only. The time the hub was last updated.</rdfs:comment>
    <rdfs:domain rdf:resource="http://example.org/onto/class/google_network_connectivity_group"/>
    <rdfs:range rdf:resource="http://www.w3.org/2001/XMLSchema#string"/>
  </owl:DatatypeProperty>
  <owl:DatatypeProperty rdf:about="http://example.org/onto/prop/google_network_connectivity_group_auto_accept_projects">
    <rdfs:label>auto_accept_projects</rdfs:label>
    <rdfs:comment>A list of project ids or project numbers for which you want to enable auto-accept. The auto-accept setting is applied to spokes being created or updated in these projects.</rdfs:comment>
    <rdfs:domain rdf:resource="http://example.org/onto/class/google_network_connectivity_group"/>
    <rdfs:range rdf:resource="http://www.w3.org/2001/XMLSchema#string"/>
  </owl:DatatypeProperty>
  <owl:DatatypeProperty rdf:about="http://example.org/onto/prop/google_network_connectivity_group_create">
    <rdfs:label>create</rdfs:label>
    <rdfs:domain rdf:resource="http://example.org/onto/class/google_network_connectivity_group"/>
    <rdfs:range rdf:resource="http://www.w3.org/2001/XMLSchema#string"/>
  </owl:DatatypeProperty>
  <owl:DatatypeProperty rdf:about="http://example.org/onto/prop/google_network_connectivity_group_delete">
    <rdfs:label>delete</rdfs:label>
    <rdfs:domain rdf:resource="http://example.org/onto/class/google_network_connectivity_group"/>
    <rdfs:range rdf:resource="http://www.w3.org/2001/XMLSchema#string"/>
  </owl:DatatypeProperty>
  <owl:DatatypeProperty rdf:about="http://example.org/onto/prop/google_network_connectivity_group_update">
    <rdfs:label>update</rdfs:label>
    <rdfs:domain rdf:resource="http://example.org/onto/class/google_network_connectivity_group"/>
    <rdfs:range rdf:resource="http://www.w3.org/2001/XMLSchema#string"/>
  </owl:DatatypeProperty>
</rdf:RDF>
