<?xml version="1.0" encoding="UTF-8"?>
<rdf:RDF
  xmlns:rdf="http://www.w3.org/1999/02/22-rdf-syntax-ns#"
  xmlns:rdfs="http://www.w3.org/2000/01/rdf-schema#"
  xmlns:owl="http://www.w3.org/2002/07/owl#"
  xmlns:xsd="http://www.w3.org/2001/XMLSchema#"
  xml:base="http://example.org/onto/">
  <owl:Class rdf:about="http://example.org/onto/class/google_chronicle_reference_list">
    <rdfs:label>google_chronicle_reference_list</rdfs:label>
    <rdfs:comment>#
#     ***     AUTO GENERATED CODE    ***    Type: MMv1     ***
#
# ----------------------------------------------------------------------------
#
#     This code is generated by Magic Modules using the following:
#
#     Configuration: https:#github.com/GoogleCloudPlatform/magic-modules/tree/main/mmv1/products/chronicle/ReferenceList.yaml
#     Template:      https:#github.com/GoogleCloudPlatform/magic-modules/tree/main/mmv1/templates/terraform/resource.html.markdown.tmpl
#
#     DO NOT EDIT this file directly. Any changes made to this file will be
#     overwritten during the next generation cycle.
#
# ----------------------------------------------------------------------------
subcategory: "Chronicle"
description: |-
  Reference lists are user-defined lists of values which users can use in multiple Rules.
---</rdfs:comment>
  </owl:Class>
  <owl:DatatypeProperty rdf:about="http://example.org/onto/prop/google_chronicle_reference_list_description">
    <rdfs:label>description</rdfs:label>
    <rdfs:comment>Required. A user-provided description of the reference list.</rdfs:comment>
    <rdfs:domain rdf:resource="http://example.org/onto/class/google_chronicle_reference_list"/>
    <rdfs:range rdf:resource="http://www.w3.org/2001/XMLSchema#string"/>
  </owl:DatatypeProperty>
  <owl:DatatypeProperty rdf:about="http://example.org/onto/prop/google_chronicle_reference_list_display_name">
    <rdfs:label>display_name</rdfs:label>
    <rdfs:comment>Output only. The unique display name of the reference list.</rdfs:comment>
    <rdfs:domain rdf:resource="http://example.org/onto/class/google_chronicle_reference_list"/>
    <rdfs:range rdf:resource="http://www.w3.org/2001/XMLSchema#string"/>
  </owl:DatatypeProperty>
  <owl:DatatypeProperty rdf:about="http://example.org/onto/prop/google_chronicle_reference_list_id">
    <rdfs:label>id</rdfs:label>
    <rdfs:domain rdf:resource="http://example.org/onto/class/google_chronicle_reference_list"/>
    <rdfs:range rdf:resource="http://www.w3.org/2001/XMLSchema#string"/>
  </owl:DatatypeProperty>
  <owl:DatatypeProperty rdf:about="http://example.org/onto/prop/google_chronicle_reference_list_instance">
    <rdfs:label>instance</rdfs:label>
    <rdfs:comment>The unique identifier for the Chronicle instance, which is the same as the customer ID.</rdfs:comment>
    <rdfs:domain rdf:resource="http://example.org/onto/class/google_chronicle_reference_list"/>
    <rdfs:range rdf:resource="http://www.w3.org/2001/XMLSchema#string"/>
  </owl:DatatypeProperty>
  <owl:DatatypeProperty rdf:about="http://example.org/onto/prop/google_chronicle_reference_list_location">
    <rdfs:label>location</rdfs:label>
    <rdfs:comment>The location of the resource. This is the geographical region where the Chronicle instance resides, such as "us" or "europe-west2".</rdfs:comment>
    <rdfs:domain rdf:resource="http://example.org/onto/class/google_chronicle_reference_list"/>
    <rdfs:range rdf:resource="http://www.w3.org/2001/XMLSchema#string"/>
  </owl:DatatypeProperty>
  <owl:DatatypeProperty rdf:about="http://example.org/onto/prop/google_chronicle_reference_list_name">
    <rdfs:label>name</rdfs:label>
    <rdfs:comment>Output only. The resource name of the reference list.
Format:
projects/{project}/locations/{location}/instances/{instance}/referenceLists/{reference_list}</rdfs:comment>
    <rdfs:domain rdf:resource="http://example.org/onto/class/google_chronicle_reference_list"/>
    <rdfs:range rdf:resource="http://www.w3.org/2001/XMLSchema#string"/>
  </owl:DatatypeProperty>
  <owl:DatatypeProperty rdf:about="http://example.org/onto/prop/google_chronicle_reference_list_project">
    <rdfs:label>project</rdfs:label>
    <rdfs:domain rdf:resource="http://example.org/onto/class/google_chronicle_reference_list"/>
    <rdfs:range rdf:resource="http://www.w3.org/2001/XMLSchema#string"/>
  </owl:DatatypeProperty>
  <owl:DatatypeProperty rdf:about="http://example.org/onto/prop/google_chronicle_reference_list_reference_list_id">
    <rdfs:label>reference_list_id</rdfs:label>
    <rdfs:comment>Required. The ID to use for the reference list. This is also the display name for
the reference list. It must satisfy the following requirements:
- Starts with letter.
- Contains only letters, numbers and underscore.
- Has length < 256.
- Must be unique.</rdfs:comment>
    <rdfs:domain rdf:resource="http://example.org/onto/class/google_chronicle_reference_list"/>
    <rdfs:range rdf:resource="http://www.w3.org/2001/XMLSchema#string"/>
  </owl:DatatypeProperty>
  <owl:DatatypeProperty rdf:about="http://example.org/onto/prop/google_chronicle_reference_list_revision_create_time">
    <rdfs:label>revision_create_time</rdfs:label>
    <rdfs:comment>Output only. The timestamp when the reference list was last updated.</rdfs:comment>
    <rdfs:domain rdf:resource="http://example.org/onto/class/google_chronicle_reference_list"/>
    <rdfs:range rdf:resource="http://www.w3.org/2001/XMLSchema#string"/>
  </owl:DatatypeProperty>
  <owl:DatatypeProperty rdf:about="http://example.org/onto/prop/google_chronicle_reference_list_rule_associations_count">
    <rdfs:label>rule_associations_count</rdfs:label>
    <rdfs:comment>Output only. The count of self-authored rules using the reference list.</rdfs:comment>
    <rdfs:domain rdf:resource="http://example.org/onto/class/google_chronicle_reference_list"/>
    <rdfs:range rdf:resource="http://www.w3.org/2001/XMLSchema#string"/>
  </owl:DatatypeProperty>
  <owl:DatatypeProperty rdf:about="http://example.org/onto/prop/google_chronicle_reference_list_rules">
    <rdfs:label>rules</rdfs:label>
    <rdfs:comment>Output only. The resource names for the associated self-authored Rules that use this
reference list.
This is returned only when the view is REFERENCE_LIST_VIEW_FULL.</rdfs:comment>
    <rdfs:domain rdf:resource="http://example.org/onto/class/google_chronicle_reference_list"/>
    <rdfs:range rdf:resource="http://www.w3.org/2001/XMLSchema#string"/>
  </owl:DatatypeProperty>
  <owl:DatatypeProperty rdf:about="http://example.org/onto/prop/google_chronicle_reference_list_syntax_type">
    <rdfs:label>syntax_type</rdfs:label>
    <rdfs:comment>Possible values:
REFERENCE_LIST_SYNTAX_TYPE_PLAIN_TEXT_STRING
REFERENCE_LIST_SYNTAX_TYPE_REGEX
REFERENCE_LIST_SYNTAX_TYPE_CIDR</rdfs:comment>
    <rdfs:domain rdf:resource="http://example.org/onto/class/google_chronicle_reference_list"/>
    <rdfs:range rdf:resource="http://www.w3.org/2001/XMLSchema#string"/>
  </owl:DatatypeProperty>
  <owl:DatatypeProperty rdf:about="http://example.org/onto/prop/google_chronicle_reference_list_value">
    <rdfs:label>value</rdfs:label>
    <rdfs:comment>Required. The value of the entry. Maximum length is 512 characters.</rdfs:comment>
    <rdfs:domain rdf:resource="http://example.org/onto/class/google_chronicle_reference_list"/>
    <rdfs:range rdf:resource="http://www.w3.org/2001/XMLSchema#string"/>
  </owl:DatatypeProperty>
  <owl:DatatypeProperty rdf:about="http://example.org/onto/prop/google_chronicle_reference_list_scope_names">
    <rdfs:label>scope_names</rdfs:label>
    <rdfs:comment>Optional. The list of scope names of the reference list. The scope names should be
full resource names and should be of the format:
"projects/{project}/locations/{location}/instances/{instance}/dataAccessScopes/{scope_name}".</rdfs:comment>
    <rdfs:domain rdf:resource="http://example.org/onto/class/google_chronicle_reference_list"/>
    <rdfs:range rdf:resource="http://www.w3.org/2001/XMLSchema#string"/>
  </owl:DatatypeProperty>
  <owl:DatatypeProperty rdf:about="http://example.org/onto/prop/google_chronicle_reference_list_create">
    <rdfs:label>create</rdfs:label>
    <rdfs:domain rdf:resource="http://example.org/onto/class/google_chronicle_reference_list"/>
    <rdfs:range rdf:resource="http://www.w3.org/2001/XMLSchema#string"/>
  </owl:DatatypeProperty>
  <owl:DatatypeProperty rdf:about="http://example.org/onto/prop/google_chronicle_reference_list_delete">
    <rdfs:label>delete</rdfs:label>
    <rdfs:domain rdf:resource="http://example.org/onto/class/google_chronicle_reference_list"/>
    <rdfs:range rdf:resource="http://www.w3.org/2001/XMLSchema#string"/>
  </owl:DatatypeProperty>
  <owl:DatatypeProperty rdf:about="http://example.org/onto/prop/google_chronicle_reference_list_update">
    <rdfs:label>update</rdfs:label>
    <rdfs:domain rdf:resource="http://example.org/onto/class/google_chronicle_reference_list"/>
    <rdfs:range rdf:resource="http://www.w3.org/2001/XMLSchema#string"/>
  </owl:DatatypeProperty>
</rdf:RDF>
