<?xml version="1.0" encoding="UTF-8"?>
<rdf:RDF
  xmlns:rdf="http://www.w3.org/1999/02/22-rdf-syntax-ns#"
  xmlns:rdfs="http://www.w3.org/2000/01/rdf-schema#"
  xmlns:owl="http://www.w3.org/2002/07/owl#"
  xmlns:xsd="http://www.w3.org/2001/XMLSchema#"
  xml:base="http://example.org/onto/">
  <owl:Class rdf:about="http://example.org/onto/class/google_discovery_engine_data_connector">
    <rdfs:label>google_discovery_engine_data_connector</rdfs:label>
    <rdfs:comment>#
#     ***     AUTO GENERATED CODE    ***    Type: MMv1     ***
#
# ----------------------------------------------------------------------------
#
#     This code is generated by Magic Modules using the following:
#
#     Configuration: https:#github.com/GoogleCloudPlatform/magic-modules/tree/main/mmv1/products/discoveryengine/DataConnector.yaml
#     Template:      https:#github.com/GoogleCloudPlatform/magic-modules/tree/main/mmv1/templates/terraform/resource.html.markdown.tmpl
#
#     DO NOT EDIT this file directly. Any changes made to this file will be
#     overwritten during the next generation cycle.
#
# ----------------------------------------------------------------------------
subcategory: "Discovery Engine"
description: |-
  DataConnector manages the connection to external data sources for all data stores grouped
  under a Collection.
---</rdfs:comment>
  </owl:Class>
  <owl:DatatypeProperty rdf:about="http://example.org/onto/prop/google_discovery_engine_data_connector_action_state">
    <rdfs:label>action_state</rdfs:label>
    <rdfs:comment>State of the action connector. This reflects whether the action connector
is initializing, active or has encountered errors. The possible value can be:
'STATE_UNSPECIFIED', 'CREATING', 'ACTIVE', 'FAILED', 'RUNNING', 'WARNING',
'INITIALIZATION_FAILED', 'UPDATING'.</rdfs:comment>
    <rdfs:domain rdf:resource="http://example.org/onto/class/google_discovery_engine_data_connector"/>
    <rdfs:range rdf:resource="http://www.w3.org/2001/XMLSchema#string"/>
  </owl:DatatypeProperty>
  <owl:DatatypeProperty rdf:about="http://example.org/onto/prop/google_discovery_engine_data_connector_auto_run_disabled">
    <rdfs:label>auto_run_disabled</rdfs:label>
    <rdfs:comment>Indicates whether full syncs are paused for this connector</rdfs:comment>
    <rdfs:domain rdf:resource="http://example.org/onto/class/google_discovery_engine_data_connector"/>
    <rdfs:range rdf:resource="http://www.w3.org/2001/XMLSchema#string"/>
  </owl:DatatypeProperty>
  <owl:DatatypeProperty rdf:about="http://example.org/onto/prop/google_discovery_engine_data_connector_blocking_reasons">
    <rdfs:label>blocking_reasons</rdfs:label>
    <rdfs:comment>User actions that must be completed before the connector can start syncing data.
The possible values can be: 'ALLOWLIST_STATIC_IP', 'ALLOWLIST_IN_SERVICE_ATTACHMENT'.</rdfs:comment>
    <rdfs:domain rdf:resource="http://example.org/onto/class/google_discovery_engine_data_connector"/>
    <rdfs:range rdf:resource="http://www.w3.org/2001/XMLSchema#string"/>
  </owl:DatatypeProperty>
  <owl:DatatypeProperty rdf:about="http://example.org/onto/prop/google_discovery_engine_data_connector_collection_display_name">
    <rdfs:label>collection_display_name</rdfs:label>
    <rdfs:comment>The display name of the Collection.
Should be human readable, used to display collections in the Console
Dashboard. UTF-8 encoded string with limit of 1024 characters.</rdfs:comment>
    <rdfs:domain rdf:resource="http://example.org/onto/class/google_discovery_engine_data_connector"/>
    <rdfs:range rdf:resource="http://www.w3.org/2001/XMLSchema#string"/>
  </owl:DatatypeProperty>
  <owl:DatatypeProperty rdf:about="http://example.org/onto/prop/google_discovery_engine_data_connector_collection_id">
    <rdfs:label>collection_id</rdfs:label>
    <rdfs:comment>The ID to use for the Collection, which will become the final component
of the Collection's resource name. A new Collection is created as
part of the DataConnector setup. DataConnector is a singleton
resource under Collection, managing all DataStores of the Collection.
This field must conform to [RFC-1034](https://tools.ietf.org/html/rfc1034)
standard with a length limit of 63 characters. Otherwise, an
INVALID_ARGUMENT error is returned.</rdfs:comment>
    <rdfs:domain rdf:resource="http://example.org/onto/class/google_discovery_engine_data_connector"/>
    <rdfs:range rdf:resource="http://www.w3.org/2001/XMLSchema#string"/>
  </owl:DatatypeProperty>
  <owl:DatatypeProperty rdf:about="http://example.org/onto/prop/google_discovery_engine_data_connector_connector_modes">
    <rdfs:label>connector_modes</rdfs:label>
    <rdfs:comment>The modes enabled for this connector. The possible value can be:
'DATA_INGESTION', 'ACTIONS', 'FEDERATED'
'EUA', 'FEDERATED_AND_EUA'.</rdfs:comment>
    <rdfs:domain rdf:resource="http://example.org/onto/class/google_discovery_engine_data_connector"/>
    <rdfs:range rdf:resource="http://www.w3.org/2001/XMLSchema#string"/>
  </owl:DatatypeProperty>
  <owl:DatatypeProperty rdf:about="http://example.org/onto/prop/google_discovery_engine_data_connector_connector_type">
    <rdfs:label>connector_type</rdfs:label>
    <rdfs:comment>The type of connector. Each source can only map to one type.
For example, salesforce, confluence and jira have THIRD_PARTY connector
type. It is not mutable once set by system. The possible value can be:
'CONNECTOR_TYPE_UNSPECIFIED', 'THIRD_PARTY', 'GCP_FHIR', 'BIG_QUERY',
'GCS', 'GOOGLE_MAIL', 'GOOGLE_CALENDAR', 'GOOGLE_DRIVE',
'NATIVE_CLOUD_IDENTITY', 'THIRD_PARTY_FEDERATED', 'THIRD_PARTY_EUA', 'GCNV'.</rdfs:comment>
    <rdfs:domain rdf:resource="http://example.org/onto/class/google_discovery_engine_data_connector"/>
    <rdfs:range rdf:resource="http://www.w3.org/2001/XMLSchema#string"/>
  </owl:DatatypeProperty>
  <owl:DatatypeProperty rdf:about="http://example.org/onto/prop/google_discovery_engine_data_connector_create_time">
    <rdfs:label>create_time</rdfs:label>
    <rdfs:comment>Timestamp when the DataConnector was created.</rdfs:comment>
    <rdfs:domain rdf:resource="http://example.org/onto/class/google_discovery_engine_data_connector"/>
    <rdfs:range rdf:resource="http://www.w3.org/2001/XMLSchema#string"/>
  </owl:DatatypeProperty>
  <owl:DatatypeProperty rdf:about="http://example.org/onto/prop/google_discovery_engine_data_connector_data_source">
    <rdfs:label>data_source</rdfs:label>
    <rdfs:comment>The name of the data source.
Supported values: 'salesforce', 'jira', 'confluence', 'bigquery'.</rdfs:comment>
    <rdfs:domain rdf:resource="http://example.org/onto/class/google_discovery_engine_data_connector"/>
    <rdfs:range rdf:resource="http://www.w3.org/2001/XMLSchema#string"/>
  </owl:DatatypeProperty>
  <owl:DatatypeProperty rdf:about="http://example.org/onto/prop/google_discovery_engine_data_connector_errors">
    <rdfs:label>errors</rdfs:label>
    <rdfs:comment>The errors from initialization or from the latest connector run.</rdfs:comment>
    <rdfs:domain rdf:resource="http://example.org/onto/class/google_discovery_engine_data_connector"/>
    <rdfs:range rdf:resource="http://www.w3.org/2001/XMLSchema#string"/>
  </owl:DatatypeProperty>
  <owl:DatatypeProperty rdf:about="http://example.org/onto/prop/google_discovery_engine_data_connector_id">
    <rdfs:label>id</rdfs:label>
    <rdfs:domain rdf:resource="http://example.org/onto/class/google_discovery_engine_data_connector"/>
    <rdfs:range rdf:resource="http://www.w3.org/2001/XMLSchema#string"/>
  </owl:DatatypeProperty>
  <owl:DatatypeProperty rdf:about="http://example.org/onto/prop/google_discovery_engine_data_connector_incremental_refresh_interval">
    <rdfs:label>incremental_refresh_interval</rdfs:label>
    <rdfs:comment>The refresh interval specifically for incremental data syncs. If unset,
incremental syncs will use the default from env, set to 3hrs.
The minimum is 30 minutes and maximum is 7 days. Applicable to only 3P
connectors. When the refresh interval is
set to the same value as the incremental refresh interval, incremental
sync will be disabled.</rdfs:comment>
    <rdfs:domain rdf:resource="http://example.org/onto/class/google_discovery_engine_data_connector"/>
    <rdfs:range rdf:resource="http://www.w3.org/2001/XMLSchema#string"/>
  </owl:DatatypeProperty>
  <owl:DatatypeProperty rdf:about="http://example.org/onto/prop/google_discovery_engine_data_connector_incremental_sync_disabled">
    <rdfs:label>incremental_sync_disabled</rdfs:label>
    <rdfs:comment>Indicates whether incremental syncs are paused for this connector.</rdfs:comment>
    <rdfs:domain rdf:resource="http://example.org/onto/class/google_discovery_engine_data_connector"/>
    <rdfs:range rdf:resource="http://www.w3.org/2001/XMLSchema#string"/>
  </owl:DatatypeProperty>
  <owl:DatatypeProperty rdf:about="http://example.org/onto/prop/google_discovery_engine_data_connector_json_params">
    <rdfs:label>json_params</rdfs:label>
    <rdfs:comment>Params needed to access the source in the format of json string.</rdfs:comment>
    <rdfs:domain rdf:resource="http://example.org/onto/class/google_discovery_engine_data_connector"/>
    <rdfs:range rdf:resource="http://www.w3.org/2001/XMLSchema#string"/>
  </owl:DatatypeProperty>
  <owl:DatatypeProperty rdf:about="http://example.org/onto/prop/google_discovery_engine_data_connector_kms_key_name">
    <rdfs:label>kms_key_name</rdfs:label>
    <rdfs:comment>The KMS key to be used to protect the DataStores managed by this connector.
Must be set for requests that need to comply with CMEK Org Policy
protections.
If this field is set and processed successfully, the DataStores created by
this connector will be protected by the KMS key.</rdfs:comment>
    <rdfs:domain rdf:resource="http://example.org/onto/class/google_discovery_engine_data_connector"/>
    <rdfs:range rdf:resource="http://www.w3.org/2001/XMLSchema#string"/>
  </owl:DatatypeProperty>
  <owl:DatatypeProperty rdf:about="http://example.org/onto/prop/google_discovery_engine_data_connector_last_sync_time">
    <rdfs:label>last_sync_time</rdfs:label>
    <rdfs:comment>For periodic connectors only, the last time a data sync was completed.</rdfs:comment>
    <rdfs:domain rdf:resource="http://example.org/onto/class/google_discovery_engine_data_connector"/>
    <rdfs:range rdf:resource="http://www.w3.org/2001/XMLSchema#string"/>
  </owl:DatatypeProperty>
  <owl:DatatypeProperty rdf:about="http://example.org/onto/prop/google_discovery_engine_data_connector_latest_pause_time">
    <rdfs:label>latest_pause_time</rdfs:label>
    <rdfs:comment>The most recent timestamp when this [DataConnector][] was paused,
affecting all functionalities such as data synchronization.
Pausing a connector has the following effects:
  - All functionalities, including data synchronization, are halted.
  - Any ongoing data synchronization job will be canceled.
  - No future data synchronization runs will be scheduled nor can be
triggered.</rdfs:comment>
    <rdfs:domain rdf:resource="http://example.org/onto/class/google_discovery_engine_data_connector"/>
    <rdfs:range rdf:resource="http://www.w3.org/2001/XMLSchema#string"/>
  </owl:DatatypeProperty>
  <owl:DatatypeProperty rdf:about="http://example.org/onto/prop/google_discovery_engine_data_connector_location">
    <rdfs:label>location</rdfs:label>
    <rdfs:comment>The geographic location where the data store should reside. The value can
only be one of "global", "us" and "eu".</rdfs:comment>
    <rdfs:domain rdf:resource="http://example.org/onto/class/google_discovery_engine_data_connector"/>
    <rdfs:range rdf:resource="http://www.w3.org/2001/XMLSchema#string"/>
  </owl:DatatypeProperty>
  <owl:DatatypeProperty rdf:about="http://example.org/onto/prop/google_discovery_engine_data_connector_name">
    <rdfs:label>name</rdfs:label>
    <rdfs:comment>The full resource name of the Data Connector.
Format: 'projects/*/locations/*/collections/*/dataConnector'.</rdfs:comment>
    <rdfs:domain rdf:resource="http://example.org/onto/class/google_discovery_engine_data_connector"/>
    <rdfs:range rdf:resource="http://www.w3.org/2001/XMLSchema#string"/>
  </owl:DatatypeProperty>
  <owl:DatatypeProperty rdf:about="http://example.org/onto/prop/google_discovery_engine_data_connector_params">
    <rdfs:label>params</rdfs:label>
    <rdfs:comment>Params needed to access the source in the format of String-to-String (Key, Value) pairs.</rdfs:comment>
    <rdfs:domain rdf:resource="http://example.org/onto/class/google_discovery_engine_data_connector"/>
    <rdfs:range rdf:resource="http://www.w3.org/2001/XMLSchema#string"/>
  </owl:DatatypeProperty>
  <owl:DatatypeProperty rdf:about="http://example.org/onto/prop/google_discovery_engine_data_connector_private_connectivity_project_id">
    <rdfs:label>private_connectivity_project_id</rdfs:label>
    <rdfs:comment>The tenant project ID associated with private connectivity connectors.
This project must be allowlisted by in order for the connector to function.</rdfs:comment>
    <rdfs:domain rdf:resource="http://example.org/onto/class/google_discovery_engine_data_connector"/>
    <rdfs:range rdf:resource="http://www.w3.org/2001/XMLSchema#string"/>
  </owl:DatatypeProperty>
  <owl:DatatypeProperty rdf:about="http://example.org/onto/prop/google_discovery_engine_data_connector_project">
    <rdfs:label>project</rdfs:label>
    <rdfs:domain rdf:resource="http://example.org/onto/class/google_discovery_engine_data_connector"/>
    <rdfs:range rdf:resource="http://www.w3.org/2001/XMLSchema#string"/>
  </owl:DatatypeProperty>
  <owl:DatatypeProperty rdf:about="http://example.org/onto/prop/google_discovery_engine_data_connector_realtime_state">
    <rdfs:label>realtime_state</rdfs:label>
    <rdfs:comment>The real-time sync state. The possible values can be:
'STATE_UNSPECIFIED', 'CREATING', 'ACTIVE', 'FAILED', 'RUNNING', 'WARNING',
'INITIALIZATION_FAILED', 'UPDATING'.</rdfs:comment>
    <rdfs:domain rdf:resource="http://example.org/onto/class/google_discovery_engine_data_connector"/>
    <rdfs:range rdf:resource="http://www.w3.org/2001/XMLSchema#string"/>
  </owl:DatatypeProperty>
  <owl:DatatypeProperty rdf:about="http://example.org/onto/prop/google_discovery_engine_data_connector_refresh_interval">
    <rdfs:label>refresh_interval</rdfs:label>
    <rdfs:comment>The refresh interval for data sync. If duration is set to 0, the data will
be synced in real time. The streaming feature is not supported yet. The
minimum is 30 minutes and maximum is 7 days. When the refresh interval is
set to the same value as the incremental refresh interval, incremental
sync will be disabled.</rdfs:comment>
    <rdfs:domain rdf:resource="http://example.org/onto/class/google_discovery_engine_data_connector"/>
    <rdfs:range rdf:resource="http://www.w3.org/2001/XMLSchema#string"/>
  </owl:DatatypeProperty>
  <owl:DatatypeProperty rdf:about="http://example.org/onto/prop/google_discovery_engine_data_connector_state">
    <rdfs:label>state</rdfs:label>
    <rdfs:comment>The state of connector. The possible value can be:
'STATE_UNSPECIFIED', 'CREATING', 'ACTIVE', 'FAILED', 'RUNNING', 'WARNING',
'INITIALIZATION_FAILED', 'UPDATING'.</rdfs:comment>
    <rdfs:domain rdf:resource="http://example.org/onto/class/google_discovery_engine_data_connector"/>
    <rdfs:range rdf:resource="http://www.w3.org/2001/XMLSchema#string"/>
  </owl:DatatypeProperty>
  <owl:DatatypeProperty rdf:about="http://example.org/onto/prop/google_discovery_engine_data_connector_static_ip_addresses">
    <rdfs:label>static_ip_addresses</rdfs:label>
    <rdfs:comment>The static IP addresses used by this connector.</rdfs:comment>
    <rdfs:domain rdf:resource="http://example.org/onto/class/google_discovery_engine_data_connector"/>
    <rdfs:range rdf:resource="http://www.w3.org/2001/XMLSchema#string"/>
  </owl:DatatypeProperty>
  <owl:DatatypeProperty rdf:about="http://example.org/onto/prop/google_discovery_engine_data_connector_static_ip_enabled">
    <rdfs:label>static_ip_enabled</rdfs:label>
    <rdfs:comment>Whether customer has enabled static IP addresses for this connector.</rdfs:comment>
    <rdfs:domain rdf:resource="http://example.org/onto/class/google_discovery_engine_data_connector"/>
    <rdfs:range rdf:resource="http://www.w3.org/2001/XMLSchema#string"/>
  </owl:DatatypeProperty>
  <owl:DatatypeProperty rdf:about="http://example.org/onto/prop/google_discovery_engine_data_connector_sync_mode">
    <rdfs:label>sync_mode</rdfs:label>
    <rdfs:comment>The data synchronization mode supported by the data connector. The possible value can be:
'PERIODIC', 'STREAMING'.</rdfs:comment>
    <rdfs:domain rdf:resource="http://example.org/onto/class/google_discovery_engine_data_connector"/>
    <rdfs:range rdf:resource="http://www.w3.org/2001/XMLSchema#string"/>
  </owl:DatatypeProperty>
  <owl:DatatypeProperty rdf:about="http://example.org/onto/prop/google_discovery_engine_data_connector_update_time">
    <rdfs:label>update_time</rdfs:label>
    <rdfs:comment>Timestamp when the DataConnector was updated.</rdfs:comment>
    <rdfs:domain rdf:resource="http://example.org/onto/class/google_discovery_engine_data_connector"/>
    <rdfs:range rdf:resource="http://www.w3.org/2001/XMLSchema#string"/>
  </owl:DatatypeProperty>
  <owl:DatatypeProperty rdf:about="http://example.org/onto/prop/google_discovery_engine_data_connector_data_store">
    <rdfs:label>data_store</rdfs:label>
    <rdfs:comment>The full resource name of the associated data store for the source
entity.
Format: 'projects/*/locations/*/collections/*/dataStores/*'.
When the connector is initialized by the DataConnectorService.SetUpDataConnector
method, a DataStore is automatically created for each source entity.</rdfs:comment>
    <rdfs:domain rdf:resource="http://example.org/onto/class/google_discovery_engine_data_connector"/>
    <rdfs:range rdf:resource="http://www.w3.org/2001/XMLSchema#string"/>
  </owl:DatatypeProperty>
  <owl:DatatypeProperty rdf:about="http://example.org/onto/prop/google_discovery_engine_data_connector_entity_name">
    <rdfs:label>entity_name</rdfs:label>
    <rdfs:comment>The name of the entity. Supported values by data source:
* Salesforce: 'Lead', 'Opportunity', 'Contact', 'Account', 'Case', 'Contract', 'Campaign'
* Jira: project, issue, attachment, comment, worklog
* Confluence: 'Content', 'Space'</rdfs:comment>
    <rdfs:domain rdf:resource="http://example.org/onto/class/google_discovery_engine_data_connector"/>
    <rdfs:range rdf:resource="http://www.w3.org/2001/XMLSchema#string"/>
  </owl:DatatypeProperty>
  <owl:DatatypeProperty rdf:about="http://example.org/onto/prop/google_discovery_engine_data_connector_key_property_mappings">
    <rdfs:label>key_property_mappings</rdfs:label>
    <rdfs:comment>Attributes for indexing.
Key: Field name.
Value: The key property to map a field to, such as 'title', and
'description'. Supported key properties:
* 'title': The title for data record. This would be displayed on search
  results.
* 'description': The description for data record. This would be displayed
  on search results.</rdfs:comment>
    <rdfs:domain rdf:resource="http://example.org/onto/class/google_discovery_engine_data_connector"/>
    <rdfs:range rdf:resource="http://www.w3.org/2001/XMLSchema#string"/>
  </owl:DatatypeProperty>
  <owl:DatatypeProperty rdf:about="http://example.org/onto/prop/google_discovery_engine_data_connector_params">
    <rdfs:label>params</rdfs:label>
    <rdfs:comment>The parameters for the entity to facilitate data ingestion.</rdfs:comment>
    <rdfs:domain rdf:resource="http://example.org/onto/class/google_discovery_engine_data_connector"/>
    <rdfs:range rdf:resource="http://www.w3.org/2001/XMLSchema#string"/>
  </owl:DatatypeProperty>
  <owl:DatatypeProperty rdf:about="http://example.org/onto/prop/google_discovery_engine_data_connector_create">
    <rdfs:label>create</rdfs:label>
    <rdfs:domain rdf:resource="http://example.org/onto/class/google_discovery_engine_data_connector"/>
    <rdfs:range rdf:resource="http://www.w3.org/2001/XMLSchema#string"/>
  </owl:DatatypeProperty>
  <owl:DatatypeProperty rdf:about="http://example.org/onto/prop/google_discovery_engine_data_connector_delete">
    <rdfs:label>delete</rdfs:label>
    <rdfs:domain rdf:resource="http://example.org/onto/class/google_discovery_engine_data_connector"/>
    <rdfs:range rdf:resource="http://www.w3.org/2001/XMLSchema#string"/>
  </owl:DatatypeProperty>
  <owl:DatatypeProperty rdf:about="http://example.org/onto/prop/google_discovery_engine_data_connector_update">
    <rdfs:label>update</rdfs:label>
    <rdfs:domain rdf:resource="http://example.org/onto/class/google_discovery_engine_data_connector"/>
    <rdfs:range rdf:resource="http://www.w3.org/2001/XMLSchema#string"/>
  </owl:DatatypeProperty>
</rdf:RDF>
