<?xml version="1.0" encoding="UTF-8"?>
<rdf:RDF
  xmlns:rdf="http://www.w3.org/1999/02/22-rdf-syntax-ns#"
  xmlns:rdfs="http://www.w3.org/2000/01/rdf-schema#"
  xmlns:owl="http://www.w3.org/2002/07/owl#"
  xmlns:xsd="http://www.w3.org/2001/XMLSchema#"
  xml:base="http://example.org/onto/">
  <owl:Class rdf:about="http://example.org/onto/class/google_migration_center_preference_set">
    <rdfs:label>google_migration_center_preference_set</rdfs:label>
    <rdfs:comment>#
#     ***     AUTO GENERATED CODE    ***    Type: MMv1     ***
#
# ----------------------------------------------------------------------------
#
#     This code is generated by Magic Modules using the following:
#
#     Configuration: https:#github.com/GoogleCloudPlatform/magic-modules/tree/main/mmv1/products/migrationcenter/PreferenceSet.yaml
#     Template:      https:#github.com/GoogleCloudPlatform/magic-modules/tree/main/mmv1/templates/terraform/resource.html.markdown.tmpl
#
#     DO NOT EDIT this file directly. Any changes made to this file will be
#     overwritten during the next generation cycle.
#
# ----------------------------------------------------------------------------
subcategory: "Migration Center"
description: |-
  Manages the PreferenceSet resource.
---</rdfs:comment>
  </owl:Class>
  <owl:DatatypeProperty rdf:about="http://example.org/onto/prop/google_migration_center_preference_set_create_time">
    <rdfs:label>create_time</rdfs:label>
    <rdfs:comment>Output only. The timestamp when the preference set was created.</rdfs:comment>
    <rdfs:domain rdf:resource="http://example.org/onto/class/google_migration_center_preference_set"/>
    <rdfs:range rdf:resource="http://www.w3.org/2001/XMLSchema#string"/>
  </owl:DatatypeProperty>
  <owl:DatatypeProperty rdf:about="http://example.org/onto/prop/google_migration_center_preference_set_description">
    <rdfs:label>description</rdfs:label>
    <rdfs:comment>A description of the preference set.</rdfs:comment>
    <rdfs:domain rdf:resource="http://example.org/onto/class/google_migration_center_preference_set"/>
    <rdfs:range rdf:resource="http://www.w3.org/2001/XMLSchema#string"/>
  </owl:DatatypeProperty>
  <owl:DatatypeProperty rdf:about="http://example.org/onto/prop/google_migration_center_preference_set_display_name">
    <rdfs:label>display_name</rdfs:label>
    <rdfs:comment>User-friendly display name. Maximum length is 63 characters.</rdfs:comment>
    <rdfs:domain rdf:resource="http://example.org/onto/class/google_migration_center_preference_set"/>
    <rdfs:range rdf:resource="http://www.w3.org/2001/XMLSchema#string"/>
  </owl:DatatypeProperty>
  <owl:DatatypeProperty rdf:about="http://example.org/onto/prop/google_migration_center_preference_set_id">
    <rdfs:label>id</rdfs:label>
    <rdfs:domain rdf:resource="http://example.org/onto/class/google_migration_center_preference_set"/>
    <rdfs:range rdf:resource="http://www.w3.org/2001/XMLSchema#string"/>
  </owl:DatatypeProperty>
  <owl:DatatypeProperty rdf:about="http://example.org/onto/prop/google_migration_center_preference_set_location">
    <rdfs:label>location</rdfs:label>
    <rdfs:comment>Part of 'parent'. See documentation of 'projectsId'.</rdfs:comment>
    <rdfs:domain rdf:resource="http://example.org/onto/class/google_migration_center_preference_set"/>
    <rdfs:range rdf:resource="http://www.w3.org/2001/XMLSchema#string"/>
  </owl:DatatypeProperty>
  <owl:DatatypeProperty rdf:about="http://example.org/onto/prop/google_migration_center_preference_set_name">
    <rdfs:label>name</rdfs:label>
    <rdfs:comment>Output only. Name of the preference set.</rdfs:comment>
    <rdfs:domain rdf:resource="http://example.org/onto/class/google_migration_center_preference_set"/>
    <rdfs:range rdf:resource="http://www.w3.org/2001/XMLSchema#string"/>
  </owl:DatatypeProperty>
  <owl:DatatypeProperty rdf:about="http://example.org/onto/prop/google_migration_center_preference_set_preference_set_id">
    <rdfs:label>preference_set_id</rdfs:label>
    <rdfs:comment>Required. User specified ID for the preference set. It will become the last component of the preference set name. The ID must be unique within the project, must conform with RFC-1034, is restricted to lower-cased letters, and has a maximum length of 63 characters. The ID must match the regular expression '[a-z]([a-z0-9-]{0,61}[a-z0-9])?'.</rdfs:comment>
    <rdfs:domain rdf:resource="http://example.org/onto/class/google_migration_center_preference_set"/>
    <rdfs:range rdf:resource="http://www.w3.org/2001/XMLSchema#string"/>
  </owl:DatatypeProperty>
  <owl:DatatypeProperty rdf:about="http://example.org/onto/prop/google_migration_center_preference_set_project">
    <rdfs:label>project</rdfs:label>
    <rdfs:domain rdf:resource="http://example.org/onto/class/google_migration_center_preference_set"/>
    <rdfs:range rdf:resource="http://www.w3.org/2001/XMLSchema#string"/>
  </owl:DatatypeProperty>
  <owl:DatatypeProperty rdf:about="http://example.org/onto/prop/google_migration_center_preference_set_update_time">
    <rdfs:label>update_time</rdfs:label>
    <rdfs:comment>Output only. The timestamp when the preference set was last updated.</rdfs:comment>
    <rdfs:domain rdf:resource="http://example.org/onto/class/google_migration_center_preference_set"/>
    <rdfs:range rdf:resource="http://www.w3.org/2001/XMLSchema#string"/>
  </owl:DatatypeProperty>
  <owl:DatatypeProperty rdf:about="http://example.org/onto/prop/google_migration_center_preference_set_create">
    <rdfs:label>create</rdfs:label>
    <rdfs:domain rdf:resource="http://example.org/onto/class/google_migration_center_preference_set"/>
    <rdfs:range rdf:resource="http://www.w3.org/2001/XMLSchema#string"/>
  </owl:DatatypeProperty>
  <owl:DatatypeProperty rdf:about="http://example.org/onto/prop/google_migration_center_preference_set_delete">
    <rdfs:label>delete</rdfs:label>
    <rdfs:domain rdf:resource="http://example.org/onto/class/google_migration_center_preference_set"/>
    <rdfs:range rdf:resource="http://www.w3.org/2001/XMLSchema#string"/>
  </owl:DatatypeProperty>
  <owl:DatatypeProperty rdf:about="http://example.org/onto/prop/google_migration_center_preference_set_update">
    <rdfs:label>update</rdfs:label>
    <rdfs:domain rdf:resource="http://example.org/onto/class/google_migration_center_preference_set"/>
    <rdfs:range rdf:resource="http://www.w3.org/2001/XMLSchema#string"/>
  </owl:DatatypeProperty>
  <owl:DatatypeProperty rdf:about="http://example.org/onto/prop/google_migration_center_preference_set_commitment_plan">
    <rdfs:label>commitment_plan</rdfs:label>
    <rdfs:comment>Commitment plan to consider when calculating costs for virtual machine insights and recommendations. If you are unsure which value to set, a 3 year commitment plan is often a good value to start with. Possible values: 'COMMITMENT_PLAN_UNSPECIFIED', 'COMMITMENT_PLAN_NONE', 'COMMITMENT_PLAN_ONE_YEAR', 'COMMITMENT_PLAN_THREE_YEARS'</rdfs:comment>
    <rdfs:domain rdf:resource="http://example.org/onto/class/google_migration_center_preference_set"/>
    <rdfs:range rdf:resource="http://www.w3.org/2001/XMLSchema#string"/>
  </owl:DatatypeProperty>
  <owl:DatatypeProperty rdf:about="http://example.org/onto/prop/google_migration_center_preference_set_sizing_optimization_strategy">
    <rdfs:label>sizing_optimization_strategy</rdfs:label>
    <rdfs:comment>Sizing optimization strategy specifies the preferred strategy used when extrapolating usage data to calculate insights and recommendations for a virtual machine. If you are unsure which value to set, a moderate sizing optimization strategy is often a good value to start with. Possible values: 'SIZING_OPTIMIZATION_STRATEGY_UNSPECIFIED', 'SIZING_OPTIMIZATION_STRATEGY_SAME_AS_SOURCE', 'SIZING_OPTIMIZATION_STRATEGY_MODERATE', 'SIZING_OPTIMIZATION_STRATEGY_AGGRESSIVE'</rdfs:comment>
    <rdfs:domain rdf:resource="http://example.org/onto/class/google_migration_center_preference_set"/>
    <rdfs:range rdf:resource="http://www.w3.org/2001/XMLSchema#string"/>
  </owl:DatatypeProperty>
  <owl:DatatypeProperty rdf:about="http://example.org/onto/prop/google_migration_center_preference_set_target_product">
    <rdfs:label>target_product</rdfs:label>
    <rdfs:comment>Target product for assets using this preference set. Specify either target product or business goal, but not both. Possible values: 'COMPUTE_MIGRATION_TARGET_PRODUCT_UNSPECIFIED', 'COMPUTE_MIGRATION_TARGET_PRODUCT_COMPUTE_ENGINE', 'COMPUTE_MIGRATION_TARGET_PRODUCT_VMWARE_ENGINE', 'COMPUTE_MIGRATION_TARGET_PRODUCT_SOLE_TENANCY'</rdfs:comment>
    <rdfs:domain rdf:resource="http://example.org/onto/class/google_migration_center_preference_set"/>
    <rdfs:range rdf:resource="http://www.w3.org/2001/XMLSchema#string"/>
  </owl:DatatypeProperty>
  <owl:DatatypeProperty rdf:about="http://example.org/onto/prop/google_migration_center_preference_set_license_type">
    <rdfs:label>license_type</rdfs:label>
    <rdfs:comment>License type to consider when calculating costs for virtual machine insights and recommendations. If unspecified, costs are calculated based on the default licensing plan. Possible values: 'LICENSE_TYPE_UNSPECIFIED', 'LICENSE_TYPE_DEFAULT', 'LICENSE_TYPE_BRING_YOUR_OWN_LICENSE'</rdfs:comment>
    <rdfs:domain rdf:resource="http://example.org/onto/class/google_migration_center_preference_set"/>
    <rdfs:range rdf:resource="http://www.w3.org/2001/XMLSchema#string"/>
  </owl:DatatypeProperty>
  <owl:DatatypeProperty rdf:about="http://example.org/onto/prop/google_migration_center_preference_set_code">
    <rdfs:label>code</rdfs:label>
    <rdfs:comment>Code to identify a Compute Engine machine series. Consult https://cloud.google.com/compute/docs/machine-resource#machine_type_comparison for more details on the available series.</rdfs:comment>
    <rdfs:domain rdf:resource="http://example.org/onto/class/google_migration_center_preference_set"/>
    <rdfs:range rdf:resource="http://www.w3.org/2001/XMLSchema#string"/>
  </owl:DatatypeProperty>
  <owl:DatatypeProperty rdf:about="http://example.org/onto/prop/google_migration_center_preference_set_preferred_regions">
    <rdfs:label>preferred_regions</rdfs:label>
    <rdfs:comment>A list of preferred regions, ordered by the most preferred region first. Set only valid Google Cloud region names. See https://cloud.google.com/compute/docs/regions-zones for available regions.</rdfs:comment>
    <rdfs:domain rdf:resource="http://example.org/onto/class/google_migration_center_preference_set"/>
    <rdfs:range rdf:resource="http://www.w3.org/2001/XMLSchema#string"/>
  </owl:DatatypeProperty>
  <owl:DatatypeProperty rdf:about="http://example.org/onto/prop/google_migration_center_preference_set_commitment_plan">
    <rdfs:label>commitment_plan</rdfs:label>
    <rdfs:comment>Commitment plan to consider when calculating costs for virtual machine insights and recommendations. If you are unsure which value to set, a 3 year commitment plan is often a good value to start with. Possible values: 'COMMITMENT_PLAN_UNSPECIFIED', 'ON_DEMAND', 'COMMITMENT_1_YEAR', 'COMMITMENT_3_YEAR'</rdfs:comment>
    <rdfs:domain rdf:resource="http://example.org/onto/class/google_migration_center_preference_set"/>
    <rdfs:range rdf:resource="http://www.w3.org/2001/XMLSchema#string"/>
  </owl:DatatypeProperty>
  <owl:DatatypeProperty rdf:about="http://example.org/onto/prop/google_migration_center_preference_set_cpu_overcommit_ratio">
    <rdfs:label>cpu_overcommit_ratio</rdfs:label>
    <rdfs:comment>CPU overcommit ratio. Acceptable values are between 1.0 and 2.0 inclusive.</rdfs:comment>
    <rdfs:domain rdf:resource="http://example.org/onto/class/google_migration_center_preference_set"/>
    <rdfs:range rdf:resource="http://www.w3.org/2001/XMLSchema#string"/>
  </owl:DatatypeProperty>
  <owl:DatatypeProperty rdf:about="http://example.org/onto/prop/google_migration_center_preference_set_host_maintenance_policy">
    <rdfs:label>host_maintenance_policy</rdfs:label>
    <rdfs:comment>Sole Tenancy nodes maintenance policy. Possible values: 'HOST_MAINTENANCE_POLICY_UNSPECIFIED', 'HOST_MAINTENANCE_POLICY_DEFAULT', 'HOST_MAINTENANCE_POLICY_RESTART_IN_PLACE', 'HOST_MAINTENANCE_POLICY_MIGRATE_WITHIN_NODE_GROUP'</rdfs:comment>
    <rdfs:domain rdf:resource="http://example.org/onto/class/google_migration_center_preference_set"/>
    <rdfs:range rdf:resource="http://www.w3.org/2001/XMLSchema#string"/>
  </owl:DatatypeProperty>
  <owl:DatatypeProperty rdf:about="http://example.org/onto/prop/google_migration_center_preference_set_node_name">
    <rdfs:label>node_name</rdfs:label>
    <rdfs:comment>Name of the Sole Tenant node. Consult https://cloud.google.com/compute/docs/nodes/sole-tenant-nodes</rdfs:comment>
    <rdfs:domain rdf:resource="http://example.org/onto/class/google_migration_center_preference_set"/>
    <rdfs:range rdf:resource="http://www.w3.org/2001/XMLSchema#string"/>
  </owl:DatatypeProperty>
  <owl:DatatypeProperty rdf:about="http://example.org/onto/prop/google_migration_center_preference_set_commitment_plan">
    <rdfs:label>commitment_plan</rdfs:label>
    <rdfs:comment>Commitment plan to consider when calculating costs for virtual machine insights and recommendations. If you are unsure which value to set, a 3 year commitment plan is often a good value to start with. Possible values: 'COMMITMENT_PLAN_UNSPECIFIED', 'ON_DEMAND', 'COMMITMENT_1_YEAR_MONTHLY_PAYMENTS', 'COMMITMENT_3_YEAR_MONTHLY_PAYMENTS', 'COMMITMENT_1_YEAR_UPFRONT_PAYMENT', 'COMMITMENT_3_YEAR_UPFRONT_PAYMENT',</rdfs:comment>
    <rdfs:domain rdf:resource="http://example.org/onto/class/google_migration_center_preference_set"/>
    <rdfs:range rdf:resource="http://www.w3.org/2001/XMLSchema#string"/>
  </owl:DatatypeProperty>
  <owl:DatatypeProperty rdf:about="http://example.org/onto/prop/google_migration_center_preference_set_cpu_overcommit_ratio">
    <rdfs:label>cpu_overcommit_ratio</rdfs:label>
    <rdfs:comment>CPU overcommit ratio. Acceptable values are between 1.0 and 8.0, with 0.1 increment.</rdfs:comment>
    <rdfs:domain rdf:resource="http://example.org/onto/class/google_migration_center_preference_set"/>
    <rdfs:range rdf:resource="http://www.w3.org/2001/XMLSchema#string"/>
  </owl:DatatypeProperty>
  <owl:DatatypeProperty rdf:about="http://example.org/onto/prop/google_migration_center_preference_set_memory_overcommit_ratio">
    <rdfs:label>memory_overcommit_ratio</rdfs:label>
    <rdfs:comment>Memory overcommit ratio. Acceptable values are 1.0, 1.25, 1.5, 1.75 and 2.0.</rdfs:comment>
    <rdfs:domain rdf:resource="http://example.org/onto/class/google_migration_center_preference_set"/>
    <rdfs:range rdf:resource="http://www.w3.org/2001/XMLSchema#string"/>
  </owl:DatatypeProperty>
  <owl:DatatypeProperty rdf:about="http://example.org/onto/prop/google_migration_center_preference_set_storage_deduplication_compression_ratio">
    <rdfs:label>storage_deduplication_compression_ratio</rdfs:label>
    <rdfs:comment>The Deduplication and Compression ratio is based on the logical (Used Before) space required to store data before applying deduplication and compression, in relation to the physical (Used After) space required after applying deduplication and compression. Specifically, the ratio is the Used Before space divided by the Used After space. For example, if the Used Before space is 3 GB, but the physical Used After space is 1 GB, the deduplication and compression ratio is 3x. Acceptable values are between 1.0 and 4.0.</rdfs:comment>
    <rdfs:domain rdf:resource="http://example.org/onto/class/google_migration_center_preference_set"/>
    <rdfs:range rdf:resource="http://www.w3.org/2001/XMLSchema#string"/>
  </owl:DatatypeProperty>
</rdf:RDF>
