<?xml version="1.0" encoding="UTF-8"?>
<rdf:RDF
  xmlns:rdf="http://www.w3.org/1999/02/22-rdf-syntax-ns#"
  xmlns:rdfs="http://www.w3.org/2000/01/rdf-schema#"
  xmlns:owl="http://www.w3.org/2002/07/owl#"
  xmlns:xsd="http://www.w3.org/2001/XMLSchema#"
  xml:base="http://example.org/onto/">
  <owl:Class rdf:about="http://example.org/onto/class/google_netapp_active_directory">
    <rdfs:label>google_netapp_active_directory</rdfs:label>
    <rdfs:comment>#
#     ***     AUTO GENERATED CODE    ***    Type: MMv1     ***
#
# ----------------------------------------------------------------------------
#
#     This code is generated by Magic Modules using the following:
#
#     Configuration: https:#github.com/GoogleCloudPlatform/magic-modules/tree/main/mmv1/products/netapp/ActiveDirectory.yaml
#     Template:      https:#github.com/GoogleCloudPlatform/magic-modules/tree/main/mmv1/templates/terraform/resource.html.markdown.tmpl
#
#     DO NOT EDIT this file directly. Any changes made to this file will be
#     overwritten during the next generation cycle.
#
# ----------------------------------------------------------------------------
subcategory: "Google Cloud NetApp Volumes"
description: |-
  ActiveDirectory is the public representation of the active directory config.
---</rdfs:comment>
  </owl:Class>
  <owl:DatatypeProperty rdf:about="http://example.org/onto/prop/google_netapp_active_directory_administrators">
    <rdfs:label>administrators</rdfs:label>
    <rdfs:comment>Domain user accounts to be added to the local Administrators group of the SMB service. Comma-separated list of domain users or groups. The Domain Admin group is automatically added when the service joins your domain as a hidden group.</rdfs:comment>
    <rdfs:domain rdf:resource="http://example.org/onto/class/google_netapp_active_directory"/>
    <rdfs:range rdf:resource="http://www.w3.org/2001/XMLSchema#string"/>
  </owl:DatatypeProperty>
  <owl:DatatypeProperty rdf:about="http://example.org/onto/prop/google_netapp_active_directory_aes_encryption">
    <rdfs:label>aes_encryption</rdfs:label>
    <rdfs:comment>Enables AES-128 and AES-256 encryption for Kerberos-based communication with Active Directory.</rdfs:comment>
    <rdfs:domain rdf:resource="http://example.org/onto/class/google_netapp_active_directory"/>
    <rdfs:range rdf:resource="http://www.w3.org/2001/XMLSchema#string"/>
  </owl:DatatypeProperty>
  <owl:DatatypeProperty rdf:about="http://example.org/onto/prop/google_netapp_active_directory_backup_operators">
    <rdfs:label>backup_operators</rdfs:label>
    <rdfs:comment>Domain user/group accounts to be added to the Backup Operators group of the SMB service. The Backup Operators group allows members to backup and restore files regardless of whether they have read or write access to the files. Comma-separated list.</rdfs:comment>
    <rdfs:domain rdf:resource="http://example.org/onto/class/google_netapp_active_directory"/>
    <rdfs:range rdf:resource="http://www.w3.org/2001/XMLSchema#string"/>
  </owl:DatatypeProperty>
  <owl:DatatypeProperty rdf:about="http://example.org/onto/prop/google_netapp_active_directory_create_time">
    <rdfs:label>create_time</rdfs:label>
    <rdfs:comment>Create time of the active directory. A timestamp in RFC3339 UTC "Zulu" format. Examples: "2023-06-22T09:13:01.617Z".</rdfs:comment>
    <rdfs:domain rdf:resource="http://example.org/onto/class/google_netapp_active_directory"/>
    <rdfs:range rdf:resource="http://www.w3.org/2001/XMLSchema#string"/>
  </owl:DatatypeProperty>
  <owl:DatatypeProperty rdf:about="http://example.org/onto/prop/google_netapp_active_directory_description">
    <rdfs:label>description</rdfs:label>
    <rdfs:comment>An optional description of this resource.</rdfs:comment>
    <rdfs:domain rdf:resource="http://example.org/onto/class/google_netapp_active_directory"/>
    <rdfs:range rdf:resource="http://www.w3.org/2001/XMLSchema#string"/>
  </owl:DatatypeProperty>
  <owl:DatatypeProperty rdf:about="http://example.org/onto/prop/google_netapp_active_directory_dns">
    <rdfs:label>dns</rdfs:label>
    <rdfs:comment>Comma separated list of DNS server IP addresses for the Active Directory domain.</rdfs:comment>
    <rdfs:domain rdf:resource="http://example.org/onto/class/google_netapp_active_directory"/>
    <rdfs:range rdf:resource="http://www.w3.org/2001/XMLSchema#string"/>
  </owl:DatatypeProperty>
  <owl:DatatypeProperty rdf:about="http://example.org/onto/prop/google_netapp_active_directory_domain">
    <rdfs:label>domain</rdfs:label>
    <rdfs:comment>Fully qualified domain name for the Active Directory domain.</rdfs:comment>
    <rdfs:domain rdf:resource="http://example.org/onto/class/google_netapp_active_directory"/>
    <rdfs:range rdf:resource="http://www.w3.org/2001/XMLSchema#string"/>
  </owl:DatatypeProperty>
  <owl:DatatypeProperty rdf:about="http://example.org/onto/prop/google_netapp_active_directory_effective_labels">
    <rdfs:label>effective_labels</rdfs:label>
    <rdfs:comment>All of labels (key/value pairs) present on the resource in GCP, including the labels configured through Terraform, other clients and services.</rdfs:comment>
    <rdfs:domain rdf:resource="http://example.org/onto/class/google_netapp_active_directory"/>
    <rdfs:range rdf:resource="http://www.w3.org/2001/XMLSchema#string"/>
  </owl:DatatypeProperty>
  <owl:DatatypeProperty rdf:about="http://example.org/onto/prop/google_netapp_active_directory_encrypt_dc_connections">
    <rdfs:label>encrypt_dc_connections</rdfs:label>
    <rdfs:comment>If enabled, traffic between the SMB server to Domain Controller (DC) will be encrypted.</rdfs:comment>
    <rdfs:domain rdf:resource="http://example.org/onto/class/google_netapp_active_directory"/>
    <rdfs:range rdf:resource="http://www.w3.org/2001/XMLSchema#string"/>
  </owl:DatatypeProperty>
  <owl:DatatypeProperty rdf:about="http://example.org/onto/prop/google_netapp_active_directory_id">
    <rdfs:label>id</rdfs:label>
    <rdfs:domain rdf:resource="http://example.org/onto/class/google_netapp_active_directory"/>
    <rdfs:range rdf:resource="http://www.w3.org/2001/XMLSchema#string"/>
  </owl:DatatypeProperty>
  <owl:DatatypeProperty rdf:about="http://example.org/onto/prop/google_netapp_active_directory_kdc_hostname">
    <rdfs:label>kdc_hostname</rdfs:label>
    <rdfs:comment>Hostname of the Active Directory server used as Kerberos Key Distribution Center. Only required for volumes using kerberized NFSv4.1</rdfs:comment>
    <rdfs:domain rdf:resource="http://example.org/onto/class/google_netapp_active_directory"/>
    <rdfs:range rdf:resource="http://www.w3.org/2001/XMLSchema#string"/>
  </owl:DatatypeProperty>
  <owl:DatatypeProperty rdf:about="http://example.org/onto/prop/google_netapp_active_directory_kdc_ip">
    <rdfs:label>kdc_ip</rdfs:label>
    <rdfs:comment>IP address of the Active Directory server used as Kerberos Key Distribution Center.</rdfs:comment>
    <rdfs:domain rdf:resource="http://example.org/onto/class/google_netapp_active_directory"/>
    <rdfs:range rdf:resource="http://www.w3.org/2001/XMLSchema#string"/>
  </owl:DatatypeProperty>
  <owl:DatatypeProperty rdf:about="http://example.org/onto/prop/google_netapp_active_directory_labels">
    <rdfs:label>labels</rdfs:label>
    <rdfs:comment>Labels as key value pairs. Example: '{ "owner": "Bob", "department": "finance", "purpose": "testing" }'.


**Note**: This field is non-authoritative, and will only manage the labels present in your configuration.
Please refer to the field 'effective_labels' for all of the labels present on the resource.</rdfs:comment>
    <rdfs:domain rdf:resource="http://example.org/onto/class/google_netapp_active_directory"/>
    <rdfs:range rdf:resource="http://www.w3.org/2001/XMLSchema#string"/>
  </owl:DatatypeProperty>
  <owl:DatatypeProperty rdf:about="http://example.org/onto/prop/google_netapp_active_directory_ldap_signing">
    <rdfs:label>ldap_signing</rdfs:label>
    <rdfs:comment>Specifies whether or not the LDAP traffic needs to be signed.</rdfs:comment>
    <rdfs:domain rdf:resource="http://example.org/onto/class/google_netapp_active_directory"/>
    <rdfs:range rdf:resource="http://www.w3.org/2001/XMLSchema#string"/>
  </owl:DatatypeProperty>
  <owl:DatatypeProperty rdf:about="http://example.org/onto/prop/google_netapp_active_directory_location">
    <rdfs:label>location</rdfs:label>
    <rdfs:comment>Name of the region for the policy to apply to.</rdfs:comment>
    <rdfs:domain rdf:resource="http://example.org/onto/class/google_netapp_active_directory"/>
    <rdfs:range rdf:resource="http://www.w3.org/2001/XMLSchema#string"/>
  </owl:DatatypeProperty>
  <owl:DatatypeProperty rdf:about="http://example.org/onto/prop/google_netapp_active_directory_name">
    <rdfs:label>name</rdfs:label>
    <rdfs:comment>The resource name of the Active Directory pool. Needs to be unique per location.</rdfs:comment>
    <rdfs:domain rdf:resource="http://example.org/onto/class/google_netapp_active_directory"/>
    <rdfs:range rdf:resource="http://www.w3.org/2001/XMLSchema#string"/>
  </owl:DatatypeProperty>
  <owl:DatatypeProperty rdf:about="http://example.org/onto/prop/google_netapp_active_directory_net_bios_prefix">
    <rdfs:label>net_bios_prefix</rdfs:label>
    <rdfs:comment>NetBIOS name prefix of the server to be created.
A five-character random ID is generated automatically, for example, -6f9a, and appended to the prefix. The full UNC share path will have the following format:
'\\NetBIOS_PREFIX-ABCD.DOMAIN_NAME\SHARE_NAME'</rdfs:comment>
    <rdfs:domain rdf:resource="http://example.org/onto/class/google_netapp_active_directory"/>
    <rdfs:range rdf:resource="http://www.w3.org/2001/XMLSchema#string"/>
  </owl:DatatypeProperty>
  <owl:DatatypeProperty rdf:about="http://example.org/onto/prop/google_netapp_active_directory_nfs_users_with_ldap">
    <rdfs:label>nfs_users_with_ldap</rdfs:label>
    <rdfs:comment>Local UNIX users on clients without valid user information in Active Directory are blocked from access to LDAP enabled volumes.
This option can be used to temporarily switch such volumes to AUTH_SYS authentication (user ID + 1-16 groups).</rdfs:comment>
    <rdfs:domain rdf:resource="http://example.org/onto/class/google_netapp_active_directory"/>
    <rdfs:range rdf:resource="http://www.w3.org/2001/XMLSchema#string"/>
  </owl:DatatypeProperty>
  <owl:DatatypeProperty rdf:about="http://example.org/onto/prop/google_netapp_active_directory_organizational_unit">
    <rdfs:label>organizational_unit</rdfs:label>
    <rdfs:comment>Name of the Organizational Unit where you intend to create the computer account for NetApp Volumes.
Defaults to 'CN=Computers' if left empty.</rdfs:comment>
    <rdfs:domain rdf:resource="http://example.org/onto/class/google_netapp_active_directory"/>
    <rdfs:range rdf:resource="http://www.w3.org/2001/XMLSchema#string"/>
  </owl:DatatypeProperty>
  <owl:DatatypeProperty rdf:about="http://example.org/onto/prop/google_netapp_active_directory_password">
    <rdfs:label>password</rdfs:label>
    <rdfs:comment>Password for specified username. Note - Manual changes done to the password will not be detected. Terraform will not re-apply the password, unless you use a new password in Terraform.</rdfs:comment>
    <rdfs:domain rdf:resource="http://example.org/onto/class/google_netapp_active_directory"/>
    <rdfs:range rdf:resource="http://www.w3.org/2001/XMLSchema#string"/>
  </owl:DatatypeProperty>
  <owl:DatatypeProperty rdf:about="http://example.org/onto/prop/google_netapp_active_directory_project">
    <rdfs:label>project</rdfs:label>
    <rdfs:domain rdf:resource="http://example.org/onto/class/google_netapp_active_directory"/>
    <rdfs:range rdf:resource="http://www.w3.org/2001/XMLSchema#string"/>
  </owl:DatatypeProperty>
  <owl:DatatypeProperty rdf:about="http://example.org/onto/prop/google_netapp_active_directory_security_operators">
    <rdfs:label>security_operators</rdfs:label>
    <rdfs:comment>Domain accounts that require elevated privileges such as 'SeSecurityPrivilege' to manage security logs. Comma-separated list.</rdfs:comment>
    <rdfs:domain rdf:resource="http://example.org/onto/class/google_netapp_active_directory"/>
    <rdfs:range rdf:resource="http://www.w3.org/2001/XMLSchema#string"/>
  </owl:DatatypeProperty>
  <owl:DatatypeProperty rdf:about="http://example.org/onto/prop/google_netapp_active_directory_site">
    <rdfs:label>site</rdfs:label>
    <rdfs:comment>Specifies an Active Directory site to manage domain controller selection.
Use when Active Directory domain controllers in multiple regions are configured. Defaults to 'Default-First-Site-Name' if left empty.</rdfs:comment>
    <rdfs:domain rdf:resource="http://example.org/onto/class/google_netapp_active_directory"/>
    <rdfs:range rdf:resource="http://www.w3.org/2001/XMLSchema#string"/>
  </owl:DatatypeProperty>
  <owl:DatatypeProperty rdf:about="http://example.org/onto/prop/google_netapp_active_directory_state">
    <rdfs:label>state</rdfs:label>
    <rdfs:comment>The state of the Active Directory policy (not the Active Directory itself).</rdfs:comment>
    <rdfs:domain rdf:resource="http://example.org/onto/class/google_netapp_active_directory"/>
    <rdfs:range rdf:resource="http://www.w3.org/2001/XMLSchema#string"/>
  </owl:DatatypeProperty>
  <owl:DatatypeProperty rdf:about="http://example.org/onto/prop/google_netapp_active_directory_state_details">
    <rdfs:label>state_details</rdfs:label>
    <rdfs:comment>The state details of the Active Directory.</rdfs:comment>
    <rdfs:domain rdf:resource="http://example.org/onto/class/google_netapp_active_directory"/>
    <rdfs:range rdf:resource="http://www.w3.org/2001/XMLSchema#string"/>
  </owl:DatatypeProperty>
  <owl:DatatypeProperty rdf:about="http://example.org/onto/prop/google_netapp_active_directory_terraform_labels">
    <rdfs:label>terraform_labels</rdfs:label>
    <rdfs:comment>The combination of labels configured directly on the resource
 and default labels configured on the provider.</rdfs:comment>
    <rdfs:domain rdf:resource="http://example.org/onto/class/google_netapp_active_directory"/>
    <rdfs:range rdf:resource="http://www.w3.org/2001/XMLSchema#string"/>
  </owl:DatatypeProperty>
  <owl:DatatypeProperty rdf:about="http://example.org/onto/prop/google_netapp_active_directory_username">
    <rdfs:label>username</rdfs:label>
    <rdfs:comment>Username for the Active Directory account with permissions to create the compute account within the specified organizational unit.</rdfs:comment>
    <rdfs:domain rdf:resource="http://example.org/onto/class/google_netapp_active_directory"/>
    <rdfs:range rdf:resource="http://www.w3.org/2001/XMLSchema#string"/>
  </owl:DatatypeProperty>
  <owl:DatatypeProperty rdf:about="http://example.org/onto/prop/google_netapp_active_directory_create">
    <rdfs:label>create</rdfs:label>
    <rdfs:domain rdf:resource="http://example.org/onto/class/google_netapp_active_directory"/>
    <rdfs:range rdf:resource="http://www.w3.org/2001/XMLSchema#string"/>
  </owl:DatatypeProperty>
  <owl:DatatypeProperty rdf:about="http://example.org/onto/prop/google_netapp_active_directory_delete">
    <rdfs:label>delete</rdfs:label>
    <rdfs:domain rdf:resource="http://example.org/onto/class/google_netapp_active_directory"/>
    <rdfs:range rdf:resource="http://www.w3.org/2001/XMLSchema#string"/>
  </owl:DatatypeProperty>
  <owl:DatatypeProperty rdf:about="http://example.org/onto/prop/google_netapp_active_directory_update">
    <rdfs:label>update</rdfs:label>
    <rdfs:domain rdf:resource="http://example.org/onto/class/google_netapp_active_directory"/>
    <rdfs:range rdf:resource="http://www.w3.org/2001/XMLSchema#string"/>
  </owl:DatatypeProperty>
</rdf:RDF>
