<?xml version="1.0" encoding="UTF-8"?>
<rdf:RDF
  xmlns:rdf="http://www.w3.org/1999/02/22-rdf-syntax-ns#"
  xmlns:rdfs="http://www.w3.org/2000/01/rdf-schema#"
  xmlns:owl="http://www.w3.org/2002/07/owl#"
  xmlns:xsd="http://www.w3.org/2001/XMLSchema#"
  xml:base="http://example.org/onto/">
  <owl:Class rdf:about="http://example.org/onto/class/google_compute_region_target_https_proxy">
    <rdfs:label>google_compute_region_target_https_proxy</rdfs:label>
    <rdfs:comment>#
#     ***     AUTO GENERATED CODE    ***    Type: MMv1     ***
#
# ----------------------------------------------------------------------------
#
#     This code is generated by Magic Modules using the following:
#
#     Configuration: https:#github.com/GoogleCloudPlatform/magic-modules/tree/main/mmv1/products/compute/RegionTargetHttpsProxy.yaml
#     Template:      https:#github.com/GoogleCloudPlatform/magic-modules/tree/main/mmv1/templates/terraform/resource.html.markdown.tmpl
#
#     DO NOT EDIT this file directly. Any changes made to this file will be
#     overwritten during the next generation cycle.
#
# ----------------------------------------------------------------------------
subcategory: "Compute Engine"
description: |-
  Represents a RegionTargetHttpsProxy resource, which is used by one or more
  forwarding rules to route incoming HTTPS requests to a URL map.
---</rdfs:comment>
  </owl:Class>
  <owl:DatatypeProperty rdf:about="http://example.org/onto/prop/google_compute_region_target_https_proxy_certificate_manager_certificates">
    <rdfs:label>certificate_manager_certificates</rdfs:label>
    <rdfs:comment>URLs to certificate manager certificate resources that are used to authenticate connections between users and the load balancer.
sslCertificates and certificateManagerCertificates can't be defined together.
Accepted format is '//certificatemanager.googleapis.com/projects/{project}/locations/{location}/certificates/{resourceName}' or just the self_link 'projects/{project}/locations/{location}/certificates/{resourceName}'</rdfs:comment>
    <rdfs:domain rdf:resource="http://example.org/onto/class/google_compute_region_target_https_proxy"/>
    <rdfs:range rdf:resource="http://www.w3.org/2001/XMLSchema#string"/>
  </owl:DatatypeProperty>
  <owl:DatatypeProperty rdf:about="http://example.org/onto/prop/google_compute_region_target_https_proxy_creation_timestamp">
    <rdfs:label>creation_timestamp</rdfs:label>
    <rdfs:comment>Creation timestamp in RFC3339 text format.</rdfs:comment>
    <rdfs:domain rdf:resource="http://example.org/onto/class/google_compute_region_target_https_proxy"/>
    <rdfs:range rdf:resource="http://www.w3.org/2001/XMLSchema#string"/>
  </owl:DatatypeProperty>
  <owl:DatatypeProperty rdf:about="http://example.org/onto/prop/google_compute_region_target_https_proxy_description">
    <rdfs:label>description</rdfs:label>
    <rdfs:comment>An optional description of this resource.</rdfs:comment>
    <rdfs:domain rdf:resource="http://example.org/onto/class/google_compute_region_target_https_proxy"/>
    <rdfs:range rdf:resource="http://www.w3.org/2001/XMLSchema#string"/>
  </owl:DatatypeProperty>
  <owl:DatatypeProperty rdf:about="http://example.org/onto/prop/google_compute_region_target_https_proxy_http_keep_alive_timeout_sec">
    <rdfs:label>http_keep_alive_timeout_sec</rdfs:label>
    <rdfs:comment>Specifies how long to keep a connection open, after completing a response,
while there is no matching traffic (in seconds). If an HTTP keepalive is
not specified, a default value (600 seconds) will be used. For Regioanl
HTTP(S) load balancer, the minimum allowed value is 5 seconds and the
maximum allowed value is 600 seconds.</rdfs:comment>
    <rdfs:domain rdf:resource="http://example.org/onto/class/google_compute_region_target_https_proxy"/>
    <rdfs:range rdf:resource="http://www.w3.org/2001/XMLSchema#string"/>
  </owl:DatatypeProperty>
  <owl:DatatypeProperty rdf:about="http://example.org/onto/prop/google_compute_region_target_https_proxy_id">
    <rdfs:label>id</rdfs:label>
    <rdfs:domain rdf:resource="http://example.org/onto/class/google_compute_region_target_https_proxy"/>
    <rdfs:range rdf:resource="http://www.w3.org/2001/XMLSchema#string"/>
  </owl:DatatypeProperty>
  <owl:DatatypeProperty rdf:about="http://example.org/onto/prop/google_compute_region_target_https_proxy_name">
    <rdfs:label>name</rdfs:label>
    <rdfs:comment>Name of the resource. Provided by the client when the resource is
created. The name must be 1-63 characters long, and comply with
RFC1035. Specifically, the name must be 1-63 characters long and match
the regular expression '[a-z]([-a-z0-9]*[a-z0-9])?' which means the
first character must be a lowercase letter, and all following
characters must be a dash, lowercase letter, or digit, except the last
character, which cannot be a dash.</rdfs:comment>
    <rdfs:domain rdf:resource="http://example.org/onto/class/google_compute_region_target_https_proxy"/>
    <rdfs:range rdf:resource="http://www.w3.org/2001/XMLSchema#string"/>
  </owl:DatatypeProperty>
  <owl:DatatypeProperty rdf:about="http://example.org/onto/prop/google_compute_region_target_https_proxy_project">
    <rdfs:label>project</rdfs:label>
    <rdfs:domain rdf:resource="http://example.org/onto/class/google_compute_region_target_https_proxy"/>
    <rdfs:range rdf:resource="http://www.w3.org/2001/XMLSchema#string"/>
  </owl:DatatypeProperty>
  <owl:DatatypeProperty rdf:about="http://example.org/onto/prop/google_compute_region_target_https_proxy_proxy_id">
    <rdfs:label>proxy_id</rdfs:label>
    <rdfs:comment>The unique identifier for the resource.</rdfs:comment>
    <rdfs:domain rdf:resource="http://example.org/onto/class/google_compute_region_target_https_proxy"/>
    <rdfs:range rdf:resource="http://www.w3.org/2001/XMLSchema#string"/>
  </owl:DatatypeProperty>
  <owl:DatatypeProperty rdf:about="http://example.org/onto/prop/google_compute_region_target_https_proxy_region">
    <rdfs:label>region</rdfs:label>
    <rdfs:comment>The Region in which the created target https proxy should reside.
If it is not provided, the provider region is used.</rdfs:comment>
    <rdfs:domain rdf:resource="http://example.org/onto/class/google_compute_region_target_https_proxy"/>
    <rdfs:range rdf:resource="http://www.w3.org/2001/XMLSchema#string"/>
  </owl:DatatypeProperty>
  <owl:DatatypeProperty rdf:about="http://example.org/onto/prop/google_compute_region_target_https_proxy_self_link">
    <rdfs:label>self_link</rdfs:label>
    <rdfs:domain rdf:resource="http://example.org/onto/class/google_compute_region_target_https_proxy"/>
    <rdfs:range rdf:resource="http://www.w3.org/2001/XMLSchema#string"/>
  </owl:DatatypeProperty>
  <owl:DatatypeProperty rdf:about="http://example.org/onto/prop/google_compute_region_target_https_proxy_server_tls_policy">
    <rdfs:label>server_tls_policy</rdfs:label>
    <rdfs:comment>A URL referring to a networksecurity.ServerTlsPolicy
resource that describes how the proxy should authenticate inbound
traffic. serverTlsPolicy only applies to a global TargetHttpsProxy
attached to globalForwardingRules with the loadBalancingScheme
set to INTERNAL_SELF_MANAGED or EXTERNAL or EXTERNAL_MANAGED.
For details which ServerTlsPolicy resources are accepted with
INTERNAL_SELF_MANAGED and which with EXTERNAL, EXTERNAL_MANAGED
loadBalancingScheme consult ServerTlsPolicy documentation.
If left blank, communications are not encrypted.

If you remove this field from your configuration at the same time as
deleting or recreating a referenced ServerTlsPolicy resource, you will
receive a resourceInUseByAnotherResource error. Use lifecycle.create_before_destroy
within the ServerTlsPolicy resource to avoid this.</rdfs:comment>
    <rdfs:domain rdf:resource="http://example.org/onto/class/google_compute_region_target_https_proxy"/>
    <rdfs:range rdf:resource="http://www.w3.org/2001/XMLSchema#string"/>
  </owl:DatatypeProperty>
  <owl:DatatypeProperty rdf:about="http://example.org/onto/prop/google_compute_region_target_https_proxy_ssl_certificates">
    <rdfs:label>ssl_certificates</rdfs:label>
    <rdfs:comment>URLs to SslCertificate resources that are used to authenticate connections between users and the load balancer.
At least one SSL certificate must be specified. Currently, you may specify up to 15 SSL certificates.
sslCertificates do not apply when the load balancing scheme is set to INTERNAL_SELF_MANAGED.</rdfs:comment>
    <rdfs:domain rdf:resource="http://example.org/onto/class/google_compute_region_target_https_proxy"/>
    <rdfs:range rdf:resource="http://www.w3.org/2001/XMLSchema#string"/>
  </owl:DatatypeProperty>
  <owl:DatatypeProperty rdf:about="http://example.org/onto/prop/google_compute_region_target_https_proxy_ssl_policy">
    <rdfs:label>ssl_policy</rdfs:label>
    <rdfs:comment>A reference to the Region SslPolicy resource that will be associated with
the TargetHttpsProxy resource. If not set, the TargetHttpsProxy
resource will not have any SSL policy configured.</rdfs:comment>
    <rdfs:domain rdf:resource="http://example.org/onto/class/google_compute_region_target_https_proxy"/>
    <rdfs:range rdf:resource="http://www.w3.org/2001/XMLSchema#string"/>
  </owl:DatatypeProperty>
  <owl:DatatypeProperty rdf:about="http://example.org/onto/prop/google_compute_region_target_https_proxy_url_map">
    <rdfs:label>url_map</rdfs:label>
    <rdfs:comment>A reference to the RegionUrlMap resource that defines the mapping from URL
to the RegionBackendService.</rdfs:comment>
    <rdfs:domain rdf:resource="http://example.org/onto/class/google_compute_region_target_https_proxy"/>
    <rdfs:range rdf:resource="http://www.w3.org/2001/XMLSchema#string"/>
  </owl:DatatypeProperty>
  <owl:DatatypeProperty rdf:about="http://example.org/onto/prop/google_compute_region_target_https_proxy_create">
    <rdfs:label>create</rdfs:label>
    <rdfs:domain rdf:resource="http://example.org/onto/class/google_compute_region_target_https_proxy"/>
    <rdfs:range rdf:resource="http://www.w3.org/2001/XMLSchema#string"/>
  </owl:DatatypeProperty>
  <owl:DatatypeProperty rdf:about="http://example.org/onto/prop/google_compute_region_target_https_proxy_delete">
    <rdfs:label>delete</rdfs:label>
    <rdfs:domain rdf:resource="http://example.org/onto/class/google_compute_region_target_https_proxy"/>
    <rdfs:range rdf:resource="http://www.w3.org/2001/XMLSchema#string"/>
  </owl:DatatypeProperty>
  <owl:DatatypeProperty rdf:about="http://example.org/onto/prop/google_compute_region_target_https_proxy_update">
    <rdfs:label>update</rdfs:label>
    <rdfs:domain rdf:resource="http://example.org/onto/class/google_compute_region_target_https_proxy"/>
    <rdfs:range rdf:resource="http://www.w3.org/2001/XMLSchema#string"/>
  </owl:DatatypeProperty>
</rdf:RDF>
