<?xml version="1.0" encoding="UTF-8"?>
<rdf:RDF
  xmlns:rdf="http://www.w3.org/1999/02/22-rdf-syntax-ns#"
  xmlns:rdfs="http://www.w3.org/2000/01/rdf-schema#"
  xmlns:owl="http://www.w3.org/2002/07/owl#"
  xmlns:xsd="http://www.w3.org/2001/XMLSchema#"
  xml:base="http://example.org/onto/">
  <owl:Class rdf:about="http://example.org/onto/class/google_logging_organization_sink">
    <rdfs:label>google_logging_organization_sink</rdfs:label>
    <rdfs:comment>#
#     ***     AUTO GENERATED CODE    ***    Type: Handwritten     ***
#
# ----------------------------------------------------------------------------
#
#     This code is generated by Magic Modules using the following:
#
#     Source file: https://github.com/GoogleCloudPlatform/magic-modules/tree/main/mmv1/third_party/terraform/website/docs/r/logging_organization_sink.html.markdown
#
#     DO NOT EDIT this file directly. Any changes made to this file will be
#     overwritten during the next generation cycle.
#
# ----------------------------------------------------------------------------
subcategory: "Cloud (Stackdriver) Logging"
description: |-
  Manages a organization-level logging sink.
---</rdfs:comment>
  </owl:Class>
  <owl:DatatypeProperty rdf:about="http://example.org/onto/prop/google_logging_organization_sink_description">
    <rdfs:label>description</rdfs:label>
    <rdfs:comment>A description of this sink. The maximum length of the description is 8000 characters.</rdfs:comment>
    <rdfs:domain rdf:resource="http://example.org/onto/class/google_logging_organization_sink"/>
    <rdfs:range rdf:resource="http://www.w3.org/2001/XMLSchema#string"/>
  </owl:DatatypeProperty>
  <owl:DatatypeProperty rdf:about="http://example.org/onto/prop/google_logging_organization_sink_destination">
    <rdfs:label>destination</rdfs:label>
    <rdfs:comment>The destination of the sink (or, in other words, where logs are written to). Can be a Cloud Storage bucket, a PubSub topic, or a BigQuery dataset. Examples: "storage.googleapis.com/[GCS_BUCKET]" "bigquery.googleapis.com/projects/[PROJECT_ID]/datasets/[DATASET]" "pubsub.googleapis.com/projects/[PROJECT_ID]/topics/[TOPIC_ID]" The writer associated with the sink must have access to write to the above resource.</rdfs:comment>
    <rdfs:domain rdf:resource="http://example.org/onto/class/google_logging_organization_sink"/>
    <rdfs:range rdf:resource="http://www.w3.org/2001/XMLSchema#string"/>
  </owl:DatatypeProperty>
  <owl:DatatypeProperty rdf:about="http://example.org/onto/prop/google_logging_organization_sink_disabled">
    <rdfs:label>disabled</rdfs:label>
    <rdfs:comment>If set to True, then this sink is disabled and it does not export any log entries.</rdfs:comment>
    <rdfs:domain rdf:resource="http://example.org/onto/class/google_logging_organization_sink"/>
    <rdfs:range rdf:resource="http://www.w3.org/2001/XMLSchema#string"/>
  </owl:DatatypeProperty>
  <owl:DatatypeProperty rdf:about="http://example.org/onto/prop/google_logging_organization_sink_filter">
    <rdfs:label>filter</rdfs:label>
    <rdfs:comment>The filter to apply when exporting logs. Only log entries that match the filter are exported.</rdfs:comment>
    <rdfs:domain rdf:resource="http://example.org/onto/class/google_logging_organization_sink"/>
    <rdfs:range rdf:resource="http://www.w3.org/2001/XMLSchema#string"/>
  </owl:DatatypeProperty>
  <owl:DatatypeProperty rdf:about="http://example.org/onto/prop/google_logging_organization_sink_id">
    <rdfs:label>id</rdfs:label>
    <rdfs:domain rdf:resource="http://example.org/onto/class/google_logging_organization_sink"/>
    <rdfs:range rdf:resource="http://www.w3.org/2001/XMLSchema#string"/>
  </owl:DatatypeProperty>
  <owl:DatatypeProperty rdf:about="http://example.org/onto/prop/google_logging_organization_sink_include_children">
    <rdfs:label>include_children</rdfs:label>
    <rdfs:comment>Whether or not to include child folders or projects in the sink export. If true, logs associated with child projects are also exported; otherwise only logs relating to the provided organization are included.</rdfs:comment>
    <rdfs:domain rdf:resource="http://example.org/onto/class/google_logging_organization_sink"/>
    <rdfs:range rdf:resource="http://www.w3.org/2001/XMLSchema#string"/>
  </owl:DatatypeProperty>
  <owl:DatatypeProperty rdf:about="http://example.org/onto/prop/google_logging_organization_sink_intercept_children">
    <rdfs:label>intercept_children</rdfs:label>
    <rdfs:comment>Whether or not to intercept logs from child projects. If true, matching logs will not match with sinks in child resources, except _Required sinks. This sink will be visible to child resources when listing sinks.</rdfs:comment>
    <rdfs:domain rdf:resource="http://example.org/onto/class/google_logging_organization_sink"/>
    <rdfs:range rdf:resource="http://www.w3.org/2001/XMLSchema#string"/>
  </owl:DatatypeProperty>
  <owl:DatatypeProperty rdf:about="http://example.org/onto/prop/google_logging_organization_sink_name">
    <rdfs:label>name</rdfs:label>
    <rdfs:comment>The name of the logging sink.</rdfs:comment>
    <rdfs:domain rdf:resource="http://example.org/onto/class/google_logging_organization_sink"/>
    <rdfs:range rdf:resource="http://www.w3.org/2001/XMLSchema#string"/>
  </owl:DatatypeProperty>
  <owl:DatatypeProperty rdf:about="http://example.org/onto/prop/google_logging_organization_sink_org_id">
    <rdfs:label>org_id</rdfs:label>
    <rdfs:comment>The numeric ID of the organization to be exported to the sink.</rdfs:comment>
    <rdfs:domain rdf:resource="http://example.org/onto/class/google_logging_organization_sink"/>
    <rdfs:range rdf:resource="http://www.w3.org/2001/XMLSchema#string"/>
  </owl:DatatypeProperty>
  <owl:DatatypeProperty rdf:about="http://example.org/onto/prop/google_logging_organization_sink_writer_identity">
    <rdfs:label>writer_identity</rdfs:label>
    <rdfs:comment>The identity associated with this sink. This identity must be granted write access to the configured destination.</rdfs:comment>
    <rdfs:domain rdf:resource="http://example.org/onto/class/google_logging_organization_sink"/>
    <rdfs:range rdf:resource="http://www.w3.org/2001/XMLSchema#string"/>
  </owl:DatatypeProperty>
  <owl:DatatypeProperty rdf:about="http://example.org/onto/prop/google_logging_organization_sink_use_partitioned_tables">
    <rdfs:label>use_partitioned_tables</rdfs:label>
    <rdfs:comment>Whether to use BigQuery's partition tables. By default, Logging creates dated tables based on the log entries' timestamps, e.g. syslog_20170523. With partitioned tables the date suffix is no longer present and special query syntax has to be used instead. In both cases, tables are sharded based on UTC timezone.</rdfs:comment>
    <rdfs:domain rdf:resource="http://example.org/onto/class/google_logging_organization_sink"/>
    <rdfs:range rdf:resource="http://www.w3.org/2001/XMLSchema#string"/>
  </owl:DatatypeProperty>
  <owl:DatatypeProperty rdf:about="http://example.org/onto/prop/google_logging_organization_sink_description">
    <rdfs:label>description</rdfs:label>
    <rdfs:comment>A description of this exclusion.</rdfs:comment>
    <rdfs:domain rdf:resource="http://example.org/onto/class/google_logging_organization_sink"/>
    <rdfs:range rdf:resource="http://www.w3.org/2001/XMLSchema#string"/>
  </owl:DatatypeProperty>
  <owl:DatatypeProperty rdf:about="http://example.org/onto/prop/google_logging_organization_sink_disabled">
    <rdfs:label>disabled</rdfs:label>
    <rdfs:comment>If set to True, then this exclusion is disabled and it does not exclude any log entries</rdfs:comment>
    <rdfs:domain rdf:resource="http://example.org/onto/class/google_logging_organization_sink"/>
    <rdfs:range rdf:resource="http://www.w3.org/2001/XMLSchema#string"/>
  </owl:DatatypeProperty>
  <owl:DatatypeProperty rdf:about="http://example.org/onto/prop/google_logging_organization_sink_filter">
    <rdfs:label>filter</rdfs:label>
    <rdfs:comment>An advanced logs filter that matches the log entries to be excluded. By using the sample function, you can exclude less than 100% of the matching log entries</rdfs:comment>
    <rdfs:domain rdf:resource="http://example.org/onto/class/google_logging_organization_sink"/>
    <rdfs:range rdf:resource="http://www.w3.org/2001/XMLSchema#string"/>
  </owl:DatatypeProperty>
  <owl:DatatypeProperty rdf:about="http://example.org/onto/prop/google_logging_organization_sink_name">
    <rdfs:label>name</rdfs:label>
    <rdfs:comment>A client-assigned identifier, such as "load-balancer-exclusion". Identifiers are limited to 100 characters and can include only letters, digits, underscores, hyphens, and periods. First character has to be alphanumeric.</rdfs:comment>
    <rdfs:domain rdf:resource="http://example.org/onto/class/google_logging_organization_sink"/>
    <rdfs:range rdf:resource="http://www.w3.org/2001/XMLSchema#string"/>
  </owl:DatatypeProperty>
</rdf:RDF>
