<?xml version="1.0" encoding="UTF-8"?>
<rdf:RDF
  xmlns:rdf="http://www.w3.org/1999/02/22-rdf-syntax-ns#"
  xmlns:rdfs="http://www.w3.org/2000/01/rdf-schema#"
  xmlns:owl="http://www.w3.org/2002/07/owl#"
  xmlns:xsd="http://www.w3.org/2001/XMLSchema#"
  xml:base="http://example.org/onto/">
  <owl:Class rdf:about="http://example.org/onto/class/google_bigtable_authorized_view">
    <rdfs:label>google_bigtable_authorized_view</rdfs:label>
    <rdfs:comment>#
#     ***     AUTO GENERATED CODE    ***    Type: Handwritten     ***
#
# ----------------------------------------------------------------------------
#
#     This code is generated by Magic Modules using the following:
#
#     Source file: https://github.com/GoogleCloudPlatform/magic-modules/tree/main/mmv1/third_party/terraform/website/docs/r/bigtable_authorized_view.html.markdown
#
#     DO NOT EDIT this file directly. Any changes made to this file will be
#     overwritten during the next generation cycle.
#
# ----------------------------------------------------------------------------
subcategory: "Cloud Bigtable"
description: |-
  Creates a Google Cloud Bigtable authorized view inside a table.
---</rdfs:comment>
  </owl:Class>
  <owl:DatatypeProperty rdf:about="http://example.org/onto/prop/google_bigtable_authorized_view_deletion_protection">
    <rdfs:label>deletion_protection</rdfs:label>
    <rdfs:comment>A field to make the authorized view protected against data loss i.e. when set to PROTECTED, deleting the authorized view, the table containing the authorized view, and the instance containing the authorized view would be prohibited.
If not provided, currently deletion protection will be set to UNPROTECTED as it is the API default value. Note this field configs the deletion protection provided by the API in the backend, and should not be confused with Terraform-side deletion protection.</rdfs:comment>
    <rdfs:domain rdf:resource="http://example.org/onto/class/google_bigtable_authorized_view"/>
    <rdfs:range rdf:resource="http://www.w3.org/2001/XMLSchema#string"/>
  </owl:DatatypeProperty>
  <owl:DatatypeProperty rdf:about="http://example.org/onto/prop/google_bigtable_authorized_view_id">
    <rdfs:label>id</rdfs:label>
    <rdfs:domain rdf:resource="http://example.org/onto/class/google_bigtable_authorized_view"/>
    <rdfs:range rdf:resource="http://www.w3.org/2001/XMLSchema#string"/>
  </owl:DatatypeProperty>
  <owl:DatatypeProperty rdf:about="http://example.org/onto/prop/google_bigtable_authorized_view_instance_name">
    <rdfs:label>instance_name</rdfs:label>
    <rdfs:comment>The name of the Bigtable instance in which the authorized view belongs.</rdfs:comment>
    <rdfs:domain rdf:resource="http://example.org/onto/class/google_bigtable_authorized_view"/>
    <rdfs:range rdf:resource="http://www.w3.org/2001/XMLSchema#string"/>
  </owl:DatatypeProperty>
  <owl:DatatypeProperty rdf:about="http://example.org/onto/prop/google_bigtable_authorized_view_name">
    <rdfs:label>name</rdfs:label>
    <rdfs:comment>The name of the authorized view. Must be 1-50 characters and must only contain hyphens, underscores, periods, letters and numbers.</rdfs:comment>
    <rdfs:domain rdf:resource="http://example.org/onto/class/google_bigtable_authorized_view"/>
    <rdfs:range rdf:resource="http://www.w3.org/2001/XMLSchema#string"/>
  </owl:DatatypeProperty>
  <owl:DatatypeProperty rdf:about="http://example.org/onto/prop/google_bigtable_authorized_view_project">
    <rdfs:label>project</rdfs:label>
    <rdfs:comment>The ID of the project in which the resource belongs. If it is not provided, the provider project is used.</rdfs:comment>
    <rdfs:domain rdf:resource="http://example.org/onto/class/google_bigtable_authorized_view"/>
    <rdfs:range rdf:resource="http://www.w3.org/2001/XMLSchema#string"/>
  </owl:DatatypeProperty>
  <owl:DatatypeProperty rdf:about="http://example.org/onto/prop/google_bigtable_authorized_view_table_name">
    <rdfs:label>table_name</rdfs:label>
    <rdfs:comment>The name of the Bigtable table in which the authorized view belongs.</rdfs:comment>
    <rdfs:domain rdf:resource="http://example.org/onto/class/google_bigtable_authorized_view"/>
    <rdfs:range rdf:resource="http://www.w3.org/2001/XMLSchema#string"/>
  </owl:DatatypeProperty>
  <owl:DatatypeProperty rdf:about="http://example.org/onto/prop/google_bigtable_authorized_view_row_prefixes">
    <rdfs:label>row_prefixes</rdfs:label>
    <rdfs:comment>Base64-encoded row prefixes to be included in the authorized view. To provide access to all rows, include the empty string as a prefix ("").</rdfs:comment>
    <rdfs:domain rdf:resource="http://example.org/onto/class/google_bigtable_authorized_view"/>
    <rdfs:range rdf:resource="http://www.w3.org/2001/XMLSchema#string"/>
  </owl:DatatypeProperty>
  <owl:DatatypeProperty rdf:about="http://example.org/onto/prop/google_bigtable_authorized_view_family_name">
    <rdfs:label>family_name</rdfs:label>
    <rdfs:comment>Name of the column family to be included in the authorized view.</rdfs:comment>
    <rdfs:domain rdf:resource="http://example.org/onto/class/google_bigtable_authorized_view"/>
    <rdfs:range rdf:resource="http://www.w3.org/2001/XMLSchema#string"/>
  </owl:DatatypeProperty>
  <owl:DatatypeProperty rdf:about="http://example.org/onto/prop/google_bigtable_authorized_view_qualifier_prefixes">
    <rdfs:label>qualifier_prefixes</rdfs:label>
    <rdfs:comment>Base64-encoded prefixes for qualifiers of the column family to be included in the authorized view. Every qualifier starting with one of these prefixes is included in the authorized view. To provide access to all qualifiers, include the empty string as a prefix ("").</rdfs:comment>
    <rdfs:domain rdf:resource="http://example.org/onto/class/google_bigtable_authorized_view"/>
    <rdfs:range rdf:resource="http://www.w3.org/2001/XMLSchema#string"/>
  </owl:DatatypeProperty>
  <owl:DatatypeProperty rdf:about="http://example.org/onto/prop/google_bigtable_authorized_view_qualifiers">
    <rdfs:label>qualifiers</rdfs:label>
    <rdfs:comment>Base64-encoded individual exact column qualifiers of the column family to be included in the authorized view.</rdfs:comment>
    <rdfs:domain rdf:resource="http://example.org/onto/class/google_bigtable_authorized_view"/>
    <rdfs:range rdf:resource="http://www.w3.org/2001/XMLSchema#string"/>
  </owl:DatatypeProperty>
  <owl:DatatypeProperty rdf:about="http://example.org/onto/prop/google_bigtable_authorized_view_create">
    <rdfs:label>create</rdfs:label>
    <rdfs:domain rdf:resource="http://example.org/onto/class/google_bigtable_authorized_view"/>
    <rdfs:range rdf:resource="http://www.w3.org/2001/XMLSchema#string"/>
  </owl:DatatypeProperty>
  <owl:DatatypeProperty rdf:about="http://example.org/onto/prop/google_bigtable_authorized_view_update">
    <rdfs:label>update</rdfs:label>
    <rdfs:domain rdf:resource="http://example.org/onto/class/google_bigtable_authorized_view"/>
    <rdfs:range rdf:resource="http://www.w3.org/2001/XMLSchema#string"/>
  </owl:DatatypeProperty>
</rdf:RDF>
