<?xml version="1.0" encoding="UTF-8"?>
<rdf:RDF
  xmlns:rdf="http://www.w3.org/1999/02/22-rdf-syntax-ns#"
  xmlns:rdfs="http://www.w3.org/2000/01/rdf-schema#"
  xmlns:owl="http://www.w3.org/2002/07/owl#"
  xmlns:xsd="http://www.w3.org/2001/XMLSchema#"
  xml:base="http://example.org/onto/">
  <owl:Class rdf:about="http://example.org/onto/class/google_edgecontainer_cluster">
    <rdfs:label>google_edgecontainer_cluster</rdfs:label>
    <rdfs:comment>#
#     ***     AUTO GENERATED CODE    ***    Type: MMv1     ***
#
# ----------------------------------------------------------------------------
#
#     This code is generated by Magic Modules using the following:
#
#     Configuration: https:#github.com/GoogleCloudPlatform/magic-modules/tree/main/mmv1/products/edgecontainer/Cluster.yaml
#     Template:      https:#github.com/GoogleCloudPlatform/magic-modules/tree/main/mmv1/templates/terraform/resource.html.markdown.tmpl
#
#     DO NOT EDIT this file directly. Any changes made to this file will be
#     overwritten during the next generation cycle.
#
# ----------------------------------------------------------------------------
subcategory: "Google Distributed Cloud Edge"
description: |-
  Cluster contains information about a Google Distributed Cloud Edge Kubernetes cluster.
---</rdfs:comment>
  </owl:Class>
  <owl:DatatypeProperty rdf:about="http://example.org/onto/prop/google_edgecontainer_cluster_cluster_ca_certificate">
    <rdfs:label>cluster_ca_certificate</rdfs:label>
    <rdfs:comment>The PEM-encoded public certificate of the cluster's CA.</rdfs:comment>
    <rdfs:domain rdf:resource="http://example.org/onto/class/google_edgecontainer_cluster"/>
    <rdfs:range rdf:resource="http://www.w3.org/2001/XMLSchema#string"/>
  </owl:DatatypeProperty>
  <owl:DatatypeProperty rdf:about="http://example.org/onto/prop/google_edgecontainer_cluster_control_plane_version">
    <rdfs:label>control_plane_version</rdfs:label>
    <rdfs:comment>The control plane release version.</rdfs:comment>
    <rdfs:domain rdf:resource="http://example.org/onto/class/google_edgecontainer_cluster"/>
    <rdfs:range rdf:resource="http://www.w3.org/2001/XMLSchema#string"/>
  </owl:DatatypeProperty>
  <owl:DatatypeProperty rdf:about="http://example.org/onto/prop/google_edgecontainer_cluster_create_time">
    <rdfs:label>create_time</rdfs:label>
    <rdfs:comment>The time the cluster was created, in RFC3339 text format.</rdfs:comment>
    <rdfs:domain rdf:resource="http://example.org/onto/class/google_edgecontainer_cluster"/>
    <rdfs:range rdf:resource="http://www.w3.org/2001/XMLSchema#string"/>
  </owl:DatatypeProperty>
  <owl:DatatypeProperty rdf:about="http://example.org/onto/prop/google_edgecontainer_cluster_default_max_pods_per_node">
    <rdfs:label>default_max_pods_per_node</rdfs:label>
    <rdfs:comment>The default maximum number of pods per node used if a maximum value is not
specified explicitly for a node pool in this cluster. If unspecified, the
Kubernetes default value will be used.</rdfs:comment>
    <rdfs:domain rdf:resource="http://example.org/onto/class/google_edgecontainer_cluster"/>
    <rdfs:range rdf:resource="http://www.w3.org/2001/XMLSchema#string"/>
  </owl:DatatypeProperty>
  <owl:DatatypeProperty rdf:about="http://example.org/onto/prop/google_edgecontainer_cluster_effective_labels">
    <rdfs:label>effective_labels</rdfs:label>
    <rdfs:comment>All of labels (key/value pairs) present on the resource in GCP, including the labels configured through Terraform, other clients and services.</rdfs:comment>
    <rdfs:domain rdf:resource="http://example.org/onto/class/google_edgecontainer_cluster"/>
    <rdfs:range rdf:resource="http://www.w3.org/2001/XMLSchema#string"/>
  </owl:DatatypeProperty>
  <owl:DatatypeProperty rdf:about="http://example.org/onto/prop/google_edgecontainer_cluster_endpoint">
    <rdfs:label>endpoint</rdfs:label>
    <rdfs:comment>The IP address of the Kubernetes API server.</rdfs:comment>
    <rdfs:domain rdf:resource="http://example.org/onto/class/google_edgecontainer_cluster"/>
    <rdfs:range rdf:resource="http://www.w3.org/2001/XMLSchema#string"/>
  </owl:DatatypeProperty>
  <owl:DatatypeProperty rdf:about="http://example.org/onto/prop/google_edgecontainer_cluster_external_load_balancer_ipv4_address_pools">
    <rdfs:label>external_load_balancer_ipv4_address_pools</rdfs:label>
    <rdfs:comment>Address pools for cluster data plane external load balancing.</rdfs:comment>
    <rdfs:domain rdf:resource="http://example.org/onto/class/google_edgecontainer_cluster"/>
    <rdfs:range rdf:resource="http://www.w3.org/2001/XMLSchema#string"/>
  </owl:DatatypeProperty>
  <owl:DatatypeProperty rdf:about="http://example.org/onto/prop/google_edgecontainer_cluster_id">
    <rdfs:label>id</rdfs:label>
    <rdfs:domain rdf:resource="http://example.org/onto/class/google_edgecontainer_cluster"/>
    <rdfs:range rdf:resource="http://www.w3.org/2001/XMLSchema#string"/>
  </owl:DatatypeProperty>
  <owl:DatatypeProperty rdf:about="http://example.org/onto/prop/google_edgecontainer_cluster_labels">
    <rdfs:label>labels</rdfs:label>
    <rdfs:comment>User-defined labels for the edgecloud cluster.

**Note**: This field is non-authoritative, and will only manage the labels present in your configuration.
Please refer to the field 'effective_labels' for all of the labels present on the resource.</rdfs:comment>
    <rdfs:domain rdf:resource="http://example.org/onto/class/google_edgecontainer_cluster"/>
    <rdfs:range rdf:resource="http://www.w3.org/2001/XMLSchema#string"/>
  </owl:DatatypeProperty>
  <owl:DatatypeProperty rdf:about="http://example.org/onto/prop/google_edgecontainer_cluster_location">
    <rdfs:label>location</rdfs:label>
    <rdfs:comment>The location of the resource.</rdfs:comment>
    <rdfs:domain rdf:resource="http://example.org/onto/class/google_edgecontainer_cluster"/>
    <rdfs:range rdf:resource="http://www.w3.org/2001/XMLSchema#string"/>
  </owl:DatatypeProperty>
  <owl:DatatypeProperty rdf:about="http://example.org/onto/prop/google_edgecontainer_cluster_maintenance_events">
    <rdfs:label>maintenance_events</rdfs:label>
    <rdfs:comment>All the maintenance events scheduled for the cluster, including the ones
ongoing, planned for the future and done in the past (up to 90 days).</rdfs:comment>
    <rdfs:domain rdf:resource="http://example.org/onto/class/google_edgecontainer_cluster"/>
    <rdfs:range rdf:resource="http://www.w3.org/2001/XMLSchema#string"/>
  </owl:DatatypeProperty>
  <owl:DatatypeProperty rdf:about="http://example.org/onto/prop/google_edgecontainer_cluster_name">
    <rdfs:label>name</rdfs:label>
    <rdfs:comment>The GDCE cluster name.</rdfs:comment>
    <rdfs:domain rdf:resource="http://example.org/onto/class/google_edgecontainer_cluster"/>
    <rdfs:range rdf:resource="http://www.w3.org/2001/XMLSchema#string"/>
  </owl:DatatypeProperty>
  <owl:DatatypeProperty rdf:about="http://example.org/onto/prop/google_edgecontainer_cluster_node_version">
    <rdfs:label>node_version</rdfs:label>
    <rdfs:comment>The lowest release version among all worker nodes. This field can be empty
if the cluster does not have any worker nodes.</rdfs:comment>
    <rdfs:domain rdf:resource="http://example.org/onto/class/google_edgecontainer_cluster"/>
    <rdfs:range rdf:resource="http://www.w3.org/2001/XMLSchema#string"/>
  </owl:DatatypeProperty>
  <owl:DatatypeProperty rdf:about="http://example.org/onto/prop/google_edgecontainer_cluster_port">
    <rdfs:label>port</rdfs:label>
    <rdfs:comment>The port number of the Kubernetes API server.</rdfs:comment>
    <rdfs:domain rdf:resource="http://example.org/onto/class/google_edgecontainer_cluster"/>
    <rdfs:range rdf:resource="http://www.w3.org/2001/XMLSchema#string"/>
  </owl:DatatypeProperty>
  <owl:DatatypeProperty rdf:about="http://example.org/onto/prop/google_edgecontainer_cluster_project">
    <rdfs:label>project</rdfs:label>
    <rdfs:domain rdf:resource="http://example.org/onto/class/google_edgecontainer_cluster"/>
    <rdfs:range rdf:resource="http://www.w3.org/2001/XMLSchema#string"/>
  </owl:DatatypeProperty>
  <owl:DatatypeProperty rdf:about="http://example.org/onto/prop/google_edgecontainer_cluster_release_channel">
    <rdfs:label>release_channel</rdfs:label>
    <rdfs:comment>The release channel a cluster is subscribed to. Possible values: ["RELEASE_CHANNEL_UNSPECIFIED", "NONE", "REGULAR"]</rdfs:comment>
    <rdfs:domain rdf:resource="http://example.org/onto/class/google_edgecontainer_cluster"/>
    <rdfs:range rdf:resource="http://www.w3.org/2001/XMLSchema#string"/>
  </owl:DatatypeProperty>
  <owl:DatatypeProperty rdf:about="http://example.org/onto/prop/google_edgecontainer_cluster_status">
    <rdfs:label>status</rdfs:label>
    <rdfs:comment>Indicates the status of the cluster.</rdfs:comment>
    <rdfs:domain rdf:resource="http://example.org/onto/class/google_edgecontainer_cluster"/>
    <rdfs:range rdf:resource="http://www.w3.org/2001/XMLSchema#string"/>
  </owl:DatatypeProperty>
  <owl:DatatypeProperty rdf:about="http://example.org/onto/prop/google_edgecontainer_cluster_target_version">
    <rdfs:label>target_version</rdfs:label>
    <rdfs:comment>The target cluster version. For example: "1.5.0".</rdfs:comment>
    <rdfs:domain rdf:resource="http://example.org/onto/class/google_edgecontainer_cluster"/>
    <rdfs:range rdf:resource="http://www.w3.org/2001/XMLSchema#string"/>
  </owl:DatatypeProperty>
  <owl:DatatypeProperty rdf:about="http://example.org/onto/prop/google_edgecontainer_cluster_terraform_labels">
    <rdfs:label>terraform_labels</rdfs:label>
    <rdfs:comment>The combination of labels configured directly on the resource
 and default labels configured on the provider.</rdfs:comment>
    <rdfs:domain rdf:resource="http://example.org/onto/class/google_edgecontainer_cluster"/>
    <rdfs:range rdf:resource="http://www.w3.org/2001/XMLSchema#string"/>
  </owl:DatatypeProperty>
  <owl:DatatypeProperty rdf:about="http://example.org/onto/prop/google_edgecontainer_cluster_update_time">
    <rdfs:label>update_time</rdfs:label>
    <rdfs:comment>The time the cluster was last updated, in RFC3339 text format.</rdfs:comment>
    <rdfs:domain rdf:resource="http://example.org/onto/class/google_edgecontainer_cluster"/>
    <rdfs:range rdf:resource="http://www.w3.org/2001/XMLSchema#string"/>
  </owl:DatatypeProperty>
  <owl:DatatypeProperty rdf:about="http://example.org/onto/prop/google_edgecontainer_cluster_username">
    <rdfs:label>username</rdfs:label>
    <rdfs:comment>An active Google username.</rdfs:comment>
    <rdfs:domain rdf:resource="http://example.org/onto/class/google_edgecontainer_cluster"/>
    <rdfs:range rdf:resource="http://www.w3.org/2001/XMLSchema#string"/>
  </owl:DatatypeProperty>
  <owl:DatatypeProperty rdf:about="http://example.org/onto/prop/google_edgecontainer_cluster_machine_filter">
    <rdfs:label>machine_filter</rdfs:label>
    <rdfs:comment>Only machines matching this filter will be allowed to host control
plane nodes. The filtering language accepts strings like "name=<name>",
and is documented here: [AIP-160](https://google.aip.dev/160).</rdfs:comment>
    <rdfs:domain rdf:resource="http://example.org/onto/class/google_edgecontainer_cluster"/>
    <rdfs:range rdf:resource="http://www.w3.org/2001/XMLSchema#string"/>
  </owl:DatatypeProperty>
  <owl:DatatypeProperty rdf:about="http://example.org/onto/prop/google_edgecontainer_cluster_node_count">
    <rdfs:label>node_count</rdfs:label>
    <rdfs:comment>The number of nodes to serve as replicas of the Control Plane.
Only 1 and 3 are supported.</rdfs:comment>
    <rdfs:domain rdf:resource="http://example.org/onto/class/google_edgecontainer_cluster"/>
    <rdfs:range rdf:resource="http://www.w3.org/2001/XMLSchema#string"/>
  </owl:DatatypeProperty>
  <owl:DatatypeProperty rdf:about="http://example.org/onto/prop/google_edgecontainer_cluster_node_location">
    <rdfs:label>node_location</rdfs:label>
    <rdfs:comment>Name of the Google Distributed Cloud Edge zones where this node pool
will be created. For example: 'us-central1-edge-customer-a'.</rdfs:comment>
    <rdfs:domain rdf:resource="http://example.org/onto/class/google_edgecontainer_cluster"/>
    <rdfs:range rdf:resource="http://www.w3.org/2001/XMLSchema#string"/>
  </owl:DatatypeProperty>
  <owl:DatatypeProperty rdf:about="http://example.org/onto/prop/google_edgecontainer_cluster_shared_deployment_policy">
    <rdfs:label>shared_deployment_policy</rdfs:label>
    <rdfs:comment>Policy configuration about how user applications are deployed. Possible values: ["SHARED_DEPLOYMENT_POLICY_UNSPECIFIED", "ALLOWED", "DISALLOWED"]</rdfs:comment>
    <rdfs:domain rdf:resource="http://example.org/onto/class/google_edgecontainer_cluster"/>
    <rdfs:range rdf:resource="http://www.w3.org/2001/XMLSchema#string"/>
  </owl:DatatypeProperty>
  <owl:DatatypeProperty rdf:about="http://example.org/onto/prop/google_edgecontainer_cluster_node_location">
    <rdfs:label>node_location</rdfs:label>
    <rdfs:comment>Name of the Google Distributed Cloud Edge zones where this node pool
will be created. For example: 'us-central1-edge-customer-a'.</rdfs:comment>
    <rdfs:domain rdf:resource="http://example.org/onto/class/google_edgecontainer_cluster"/>
    <rdfs:range rdf:resource="http://www.w3.org/2001/XMLSchema#string"/>
  </owl:DatatypeProperty>
  <owl:DatatypeProperty rdf:about="http://example.org/onto/prop/google_edgecontainer_cluster_kms_key">
    <rdfs:label>kms_key</rdfs:label>
    <rdfs:comment>The Cloud KMS CryptoKey e.g.
projects/{project}/locations/{location}/keyRings/{keyRing}/cryptoKeys/{cryptoKey}
to use for protecting control plane disks. If not specified, a
Google-managed key will be used instead.</rdfs:comment>
    <rdfs:domain rdf:resource="http://example.org/onto/class/google_edgecontainer_cluster"/>
    <rdfs:range rdf:resource="http://www.w3.org/2001/XMLSchema#string"/>
  </owl:DatatypeProperty>
  <owl:DatatypeProperty rdf:about="http://example.org/onto/prop/google_edgecontainer_cluster_kms_key_active_version">
    <rdfs:label>kms_key_active_version</rdfs:label>
    <rdfs:comment>The Cloud KMS CryptoKeyVersion currently in use for protecting control
plane disks. Only applicable if kms_key is set.</rdfs:comment>
    <rdfs:domain rdf:resource="http://example.org/onto/class/google_edgecontainer_cluster"/>
    <rdfs:range rdf:resource="http://www.w3.org/2001/XMLSchema#string"/>
  </owl:DatatypeProperty>
  <owl:DatatypeProperty rdf:about="http://example.org/onto/prop/google_edgecontainer_cluster_kms_key_state">
    <rdfs:label>kms_key_state</rdfs:label>
    <rdfs:comment>Availability of the Cloud KMS CryptoKey. If not 'KEY_AVAILABLE', then
nodes may go offline as they cannot access their local data. This can be
caused by a lack of permissions to use the key, or if the key is disabled
or deleted.</rdfs:comment>
    <rdfs:domain rdf:resource="http://example.org/onto/class/google_edgecontainer_cluster"/>
    <rdfs:range rdf:resource="http://www.w3.org/2001/XMLSchema#string"/>
  </owl:DatatypeProperty>
  <owl:DatatypeProperty rdf:about="http://example.org/onto/prop/google_edgecontainer_cluster_kms_status">
    <rdfs:label>kms_status</rdfs:label>
    <rdfs:comment>Error status returned by Cloud KMS when using this key. This field may be
populated only if 'kms_key_state' is not 'KMS_KEY_STATE_KEY_AVAILABLE'.
If populated, this field contains the error status reported by Cloud KMS.</rdfs:comment>
    <rdfs:domain rdf:resource="http://example.org/onto/class/google_edgecontainer_cluster"/>
    <rdfs:range rdf:resource="http://www.w3.org/2001/XMLSchema#string"/>
  </owl:DatatypeProperty>
  <owl:DatatypeProperty rdf:about="http://example.org/onto/prop/google_edgecontainer_cluster_membership">
    <rdfs:label>membership</rdfs:label>
    <rdfs:comment>The name of the managed Hub Membership resource associated to this cluster.
Membership names are formatted as
'projects/<project-number>/locations/global/membership/<cluster-id>'.</rdfs:comment>
    <rdfs:domain rdf:resource="http://example.org/onto/class/google_edgecontainer_cluster"/>
    <rdfs:range rdf:resource="http://www.w3.org/2001/XMLSchema#string"/>
  </owl:DatatypeProperty>
  <owl:DatatypeProperty rdf:about="http://example.org/onto/prop/google_edgecontainer_cluster_project">
    <rdfs:label>project</rdfs:label>
    <rdfs:comment>The name of the Fleet host project where this cluster will be registered.
Project names are formatted as
'projects/<project-number>'.</rdfs:comment>
    <rdfs:domain rdf:resource="http://example.org/onto/class/google_edgecontainer_cluster"/>
    <rdfs:range rdf:resource="http://www.w3.org/2001/XMLSchema#string"/>
  </owl:DatatypeProperty>
  <owl:DatatypeProperty rdf:about="http://example.org/onto/prop/google_edgecontainer_cluster_id">
    <rdfs:label>id</rdfs:label>
    <rdfs:comment>A unique (per cluster) id for the window.</rdfs:comment>
    <rdfs:domain rdf:resource="http://example.org/onto/class/google_edgecontainer_cluster"/>
    <rdfs:range rdf:resource="http://www.w3.org/2001/XMLSchema#string"/>
  </owl:DatatypeProperty>
  <owl:DatatypeProperty rdf:about="http://example.org/onto/prop/google_edgecontainer_cluster_end_time">
    <rdfs:label>end_time</rdfs:label>
    <rdfs:comment>The time that the window ends. The end time must take place after the
start time.</rdfs:comment>
    <rdfs:domain rdf:resource="http://example.org/onto/class/google_edgecontainer_cluster"/>
    <rdfs:range rdf:resource="http://www.w3.org/2001/XMLSchema#string"/>
  </owl:DatatypeProperty>
  <owl:DatatypeProperty rdf:about="http://example.org/onto/prop/google_edgecontainer_cluster_start_time">
    <rdfs:label>start_time</rdfs:label>
    <rdfs:comment>The time that the window first starts.</rdfs:comment>
    <rdfs:domain rdf:resource="http://example.org/onto/class/google_edgecontainer_cluster"/>
    <rdfs:range rdf:resource="http://www.w3.org/2001/XMLSchema#string"/>
  </owl:DatatypeProperty>
  <owl:DatatypeProperty rdf:about="http://example.org/onto/prop/google_edgecontainer_cluster_recurrence">
    <rdfs:label>recurrence</rdfs:label>
    <rdfs:comment>An RRULE (https://tools.ietf.org/html/rfc5545#section-3.8.5.3) for how
this window recurs. They go on for the span of time between the start and
end time.</rdfs:comment>
    <rdfs:domain rdf:resource="http://example.org/onto/class/google_edgecontainer_cluster"/>
    <rdfs:range rdf:resource="http://www.w3.org/2001/XMLSchema#string"/>
  </owl:DatatypeProperty>
  <owl:DatatypeProperty rdf:about="http://example.org/onto/prop/google_edgecontainer_cluster_end_time">
    <rdfs:label>end_time</rdfs:label>
    <rdfs:comment>The time that the window ends. The end time must take place after the
start time.</rdfs:comment>
    <rdfs:domain rdf:resource="http://example.org/onto/class/google_edgecontainer_cluster"/>
    <rdfs:range rdf:resource="http://www.w3.org/2001/XMLSchema#string"/>
  </owl:DatatypeProperty>
  <owl:DatatypeProperty rdf:about="http://example.org/onto/prop/google_edgecontainer_cluster_start_time">
    <rdfs:label>start_time</rdfs:label>
    <rdfs:comment>The time that the window first starts.</rdfs:comment>
    <rdfs:domain rdf:resource="http://example.org/onto/class/google_edgecontainer_cluster"/>
    <rdfs:range rdf:resource="http://www.w3.org/2001/XMLSchema#string"/>
  </owl:DatatypeProperty>
  <owl:DatatypeProperty rdf:about="http://example.org/onto/prop/google_edgecontainer_cluster_cluster_ipv4_cidr_blocks">
    <rdfs:label>cluster_ipv4_cidr_blocks</rdfs:label>
    <rdfs:comment>All pods in the cluster are assigned an RFC1918 IPv4 address from these
blocks. Only a single block is supported. This field cannot be changed
after creation.</rdfs:comment>
    <rdfs:domain rdf:resource="http://example.org/onto/class/google_edgecontainer_cluster"/>
    <rdfs:range rdf:resource="http://www.w3.org/2001/XMLSchema#string"/>
  </owl:DatatypeProperty>
  <owl:DatatypeProperty rdf:about="http://example.org/onto/prop/google_edgecontainer_cluster_cluster_ipv6_cidr_blocks">
    <rdfs:label>cluster_ipv6_cidr_blocks</rdfs:label>
    <rdfs:comment>If specified, dual stack mode is enabled and all pods in the cluster are
assigned an IPv6 address from these blocks alongside from an IPv4
address. Only a single block is supported. This field cannot be changed
after creation.</rdfs:comment>
    <rdfs:domain rdf:resource="http://example.org/onto/class/google_edgecontainer_cluster"/>
    <rdfs:range rdf:resource="http://www.w3.org/2001/XMLSchema#string"/>
  </owl:DatatypeProperty>
  <owl:DatatypeProperty rdf:about="http://example.org/onto/prop/google_edgecontainer_cluster_network_type">
    <rdfs:label>network_type</rdfs:label>
    <rdfs:comment>IP addressing type of this cluster i.e. SINGLESTACK_V4 vs DUALSTACK_V4_V6.</rdfs:comment>
    <rdfs:domain rdf:resource="http://example.org/onto/class/google_edgecontainer_cluster"/>
    <rdfs:range rdf:resource="http://www.w3.org/2001/XMLSchema#string"/>
  </owl:DatatypeProperty>
  <owl:DatatypeProperty rdf:about="http://example.org/onto/prop/google_edgecontainer_cluster_services_ipv4_cidr_blocks">
    <rdfs:label>services_ipv4_cidr_blocks</rdfs:label>
    <rdfs:comment>All services in the cluster are assigned an RFC1918 IPv4 address from these
blocks. Only a single block is supported. This field cannot be changed
after creation.</rdfs:comment>
    <rdfs:domain rdf:resource="http://example.org/onto/class/google_edgecontainer_cluster"/>
    <rdfs:range rdf:resource="http://www.w3.org/2001/XMLSchema#string"/>
  </owl:DatatypeProperty>
  <owl:DatatypeProperty rdf:about="http://example.org/onto/prop/google_edgecontainer_cluster_services_ipv6_cidr_blocks">
    <rdfs:label>services_ipv6_cidr_blocks</rdfs:label>
    <rdfs:comment>If specified, dual stack mode is enabled and all services in the cluster are
assigned an IPv6 address from these blocks alongside from an IPv4
address. Only a single block is supported. This field cannot be changed
after creation.</rdfs:comment>
    <rdfs:domain rdf:resource="http://example.org/onto/class/google_edgecontainer_cluster"/>
    <rdfs:range rdf:resource="http://www.w3.org/2001/XMLSchema#string"/>
  </owl:DatatypeProperty>
  <owl:DatatypeProperty rdf:about="http://example.org/onto/prop/google_edgecontainer_cluster_disabled">
    <rdfs:label>disabled</rdfs:label>
    <rdfs:comment>Whether Ingress is disabled.</rdfs:comment>
    <rdfs:domain rdf:resource="http://example.org/onto/class/google_edgecontainer_cluster"/>
    <rdfs:range rdf:resource="http://www.w3.org/2001/XMLSchema#string"/>
  </owl:DatatypeProperty>
  <owl:DatatypeProperty rdf:about="http://example.org/onto/prop/google_edgecontainer_cluster_ipv4_vip">
    <rdfs:label>ipv4_vip</rdfs:label>
    <rdfs:comment>Ingress VIP.</rdfs:comment>
    <rdfs:domain rdf:resource="http://example.org/onto/class/google_edgecontainer_cluster"/>
    <rdfs:range rdf:resource="http://www.w3.org/2001/XMLSchema#string"/>
  </owl:DatatypeProperty>
  <owl:DatatypeProperty rdf:about="http://example.org/onto/prop/google_edgecontainer_cluster_create">
    <rdfs:label>create</rdfs:label>
    <rdfs:domain rdf:resource="http://example.org/onto/class/google_edgecontainer_cluster"/>
    <rdfs:range rdf:resource="http://www.w3.org/2001/XMLSchema#string"/>
  </owl:DatatypeProperty>
  <owl:DatatypeProperty rdf:about="http://example.org/onto/prop/google_edgecontainer_cluster_delete">
    <rdfs:label>delete</rdfs:label>
    <rdfs:domain rdf:resource="http://example.org/onto/class/google_edgecontainer_cluster"/>
    <rdfs:range rdf:resource="http://www.w3.org/2001/XMLSchema#string"/>
  </owl:DatatypeProperty>
  <owl:DatatypeProperty rdf:about="http://example.org/onto/prop/google_edgecontainer_cluster_update">
    <rdfs:label>update</rdfs:label>
    <rdfs:domain rdf:resource="http://example.org/onto/class/google_edgecontainer_cluster"/>
    <rdfs:range rdf:resource="http://www.w3.org/2001/XMLSchema#string"/>
  </owl:DatatypeProperty>
</rdf:RDF>
