<?xml version="1.0" encoding="UTF-8"?>
<rdf:RDF
  xmlns:rdf="http://www.w3.org/1999/02/22-rdf-syntax-ns#"
  xmlns:rdfs="http://www.w3.org/2000/01/rdf-schema#"
  xmlns:owl="http://www.w3.org/2002/07/owl#"
  xmlns:xsd="http://www.w3.org/2001/XMLSchema#"
  xml:base="http://example.org/onto/">
  <owl:Class rdf:about="http://example.org/onto/class/google_billing_budget">
    <rdfs:label>google_billing_budget</rdfs:label>
    <rdfs:comment>#
#     ***     AUTO GENERATED CODE    ***    Type: MMv1     ***
#
# ----------------------------------------------------------------------------
#
#     This code is generated by Magic Modules using the following:
#
#     Configuration: https:#github.com/GoogleCloudPlatform/magic-modules/tree/main/mmv1/products/billingbudget/Budget.yaml
#     Template:      https:#github.com/GoogleCloudPlatform/magic-modules/tree/main/mmv1/templates/terraform/resource.html.markdown.tmpl
#
#     DO NOT EDIT this file directly. Any changes made to this file will be
#     overwritten during the next generation cycle.
#
# ----------------------------------------------------------------------------
subcategory: "Cloud Billing"
description: |-
  Budget configuration for a billing account.
---</rdfs:comment>
  </owl:Class>
  <owl:DatatypeProperty rdf:about="http://example.org/onto/prop/google_billing_budget_billing_account">
    <rdfs:label>billing_account</rdfs:label>
    <rdfs:comment>ID of the billing account to set a budget on.</rdfs:comment>
    <rdfs:domain rdf:resource="http://example.org/onto/class/google_billing_budget"/>
    <rdfs:range rdf:resource="http://www.w3.org/2001/XMLSchema#string"/>
  </owl:DatatypeProperty>
  <owl:DatatypeProperty rdf:about="http://example.org/onto/prop/google_billing_budget_display_name">
    <rdfs:label>display_name</rdfs:label>
    <rdfs:comment>User data for display name in UI. Must be <= 60 chars.</rdfs:comment>
    <rdfs:domain rdf:resource="http://example.org/onto/class/google_billing_budget"/>
    <rdfs:range rdf:resource="http://www.w3.org/2001/XMLSchema#string"/>
  </owl:DatatypeProperty>
  <owl:DatatypeProperty rdf:about="http://example.org/onto/prop/google_billing_budget_id">
    <rdfs:label>id</rdfs:label>
    <rdfs:domain rdf:resource="http://example.org/onto/class/google_billing_budget"/>
    <rdfs:range rdf:resource="http://www.w3.org/2001/XMLSchema#string"/>
  </owl:DatatypeProperty>
  <owl:DatatypeProperty rdf:about="http://example.org/onto/prop/google_billing_budget_name">
    <rdfs:label>name</rdfs:label>
    <rdfs:comment>Resource name of the budget. The resource name
implies the scope of a budget. Values are of the form
billingAccounts/{billingAccountId}/budgets/{budgetId}.</rdfs:comment>
    <rdfs:domain rdf:resource="http://example.org/onto/class/google_billing_budget"/>
    <rdfs:range rdf:resource="http://www.w3.org/2001/XMLSchema#string"/>
  </owl:DatatypeProperty>
  <owl:DatatypeProperty rdf:about="http://example.org/onto/prop/google_billing_budget_ownership_scope">
    <rdfs:label>ownership_scope</rdfs:label>
    <rdfs:comment>The ownership scope of the budget. The ownership scope and users'
IAM permissions determine who has full access to the budget's data. Possible values: ["OWNERSHIP_SCOPE_UNSPECIFIED", "ALL_USERS", "BILLING_ACCOUNT"]</rdfs:comment>
    <rdfs:domain rdf:resource="http://example.org/onto/class/google_billing_budget"/>
    <rdfs:range rdf:resource="http://www.w3.org/2001/XMLSchema#string"/>
  </owl:DatatypeProperty>
  <owl:DatatypeProperty rdf:about="http://example.org/onto/prop/google_billing_budget_disable_default_iam_recipients">
    <rdfs:label>disable_default_iam_recipients</rdfs:label>
    <rdfs:comment>Boolean. When set to true, disables default notifications sent
when a threshold is exceeded. Default recipients are
those with Billing Account Administrators and Billing
Account Users IAM roles for the target account.</rdfs:comment>
    <rdfs:domain rdf:resource="http://example.org/onto/class/google_billing_budget"/>
    <rdfs:range rdf:resource="http://www.w3.org/2001/XMLSchema#string"/>
  </owl:DatatypeProperty>
  <owl:DatatypeProperty rdf:about="http://example.org/onto/prop/google_billing_budget_enable_project_level_recipients">
    <rdfs:label>enable_project_level_recipients</rdfs:label>
    <rdfs:comment>When set to true, and when the budget has a single project configured,
notifications will be sent to project level recipients of that project.
This field will be ignored if the budget has multiple or no project configured.

Currently, project level recipients are the users with Owner role on a cloud project.</rdfs:comment>
    <rdfs:domain rdf:resource="http://example.org/onto/class/google_billing_budget"/>
    <rdfs:range rdf:resource="http://www.w3.org/2001/XMLSchema#string"/>
  </owl:DatatypeProperty>
  <owl:DatatypeProperty rdf:about="http://example.org/onto/prop/google_billing_budget_monitoring_notification_channels">
    <rdfs:label>monitoring_notification_channels</rdfs:label>
    <rdfs:comment>The full resource name of a monitoring notification
channel in the form
projects/{project_id}/notificationChannels/{channel_id}.
A maximum of 5 channels are allowed.</rdfs:comment>
    <rdfs:domain rdf:resource="http://example.org/onto/class/google_billing_budget"/>
    <rdfs:range rdf:resource="http://www.w3.org/2001/XMLSchema#string"/>
  </owl:DatatypeProperty>
  <owl:DatatypeProperty rdf:about="http://example.org/onto/prop/google_billing_budget_pubsub_topic">
    <rdfs:label>pubsub_topic</rdfs:label>
    <rdfs:comment>The name of the Cloud Pub/Sub topic where budget related
messages will be published, in the form
projects/{project_id}/topics/{topic_id}. Updates are sent
at regular intervals to the topic.</rdfs:comment>
    <rdfs:domain rdf:resource="http://example.org/onto/class/google_billing_budget"/>
    <rdfs:range rdf:resource="http://www.w3.org/2001/XMLSchema#string"/>
  </owl:DatatypeProperty>
  <owl:DatatypeProperty rdf:about="http://example.org/onto/prop/google_billing_budget_schema_version">
    <rdfs:label>schema_version</rdfs:label>
    <rdfs:comment>The schema version of the notification. Only "1.0" is
accepted. It represents the JSON schema as defined in
https://cloud.google.com/billing/docs/how-to/budgets#notification_format.</rdfs:comment>
    <rdfs:domain rdf:resource="http://example.org/onto/class/google_billing_budget"/>
    <rdfs:range rdf:resource="http://www.w3.org/2001/XMLSchema#string"/>
  </owl:DatatypeProperty>
  <owl:DatatypeProperty rdf:about="http://example.org/onto/prop/google_billing_budget_last_period_amount">
    <rdfs:label>last_period_amount</rdfs:label>
    <rdfs:comment>Configures a budget amount that is automatically set to 100% of
last period's spend.
Boolean. Set value to true to use. Do not set to false, instead
use the 'specified_amount' block.</rdfs:comment>
    <rdfs:domain rdf:resource="http://example.org/onto/class/google_billing_budget"/>
    <rdfs:range rdf:resource="http://www.w3.org/2001/XMLSchema#string"/>
  </owl:DatatypeProperty>
  <owl:DatatypeProperty rdf:about="http://example.org/onto/prop/google_billing_budget_currency_code">
    <rdfs:label>currency_code</rdfs:label>
    <rdfs:comment>The 3-letter currency code defined in ISO 4217.</rdfs:comment>
    <rdfs:domain rdf:resource="http://example.org/onto/class/google_billing_budget"/>
    <rdfs:range rdf:resource="http://www.w3.org/2001/XMLSchema#string"/>
  </owl:DatatypeProperty>
  <owl:DatatypeProperty rdf:about="http://example.org/onto/prop/google_billing_budget_nanos">
    <rdfs:label>nanos</rdfs:label>
    <rdfs:comment>Number of nano (10^-9) units of the amount.
The value must be between -999,999,999 and +999,999,999
inclusive. If units is positive, nanos must be positive or
zero. If units is zero, nanos can be positive, zero, or
negative. If units is negative, nanos must be negative or
zero. For example $-1.75 is represented as units=-1 and
nanos=-750,000,000.</rdfs:comment>
    <rdfs:domain rdf:resource="http://example.org/onto/class/google_billing_budget"/>
    <rdfs:range rdf:resource="http://www.w3.org/2001/XMLSchema#string"/>
  </owl:DatatypeProperty>
  <owl:DatatypeProperty rdf:about="http://example.org/onto/prop/google_billing_budget_units">
    <rdfs:label>units</rdfs:label>
    <rdfs:comment>The whole units of the amount. For example if currencyCode
is "USD", then 1 unit is one US dollar.</rdfs:comment>
    <rdfs:domain rdf:resource="http://example.org/onto/class/google_billing_budget"/>
    <rdfs:range rdf:resource="http://www.w3.org/2001/XMLSchema#string"/>
  </owl:DatatypeProperty>
  <owl:DatatypeProperty rdf:about="http://example.org/onto/prop/google_billing_budget_calendar_period">
    <rdfs:label>calendar_period</rdfs:label>
    <rdfs:comment>A CalendarPeriod represents the abstract concept of a recurring time period that has a
canonical start. Grammatically, "the start of the current CalendarPeriod".
All calendar times begin at 12 AM US and Canadian Pacific Time (UTC-8).

Exactly one of 'calendar_period', 'custom_period' must be provided. Possible values: ["MONTH", "QUARTER", "YEAR", "CALENDAR_PERIOD_UNSPECIFIED"]</rdfs:comment>
    <rdfs:domain rdf:resource="http://example.org/onto/class/google_billing_budget"/>
    <rdfs:range rdf:resource="http://www.w3.org/2001/XMLSchema#string"/>
  </owl:DatatypeProperty>
  <owl:DatatypeProperty rdf:about="http://example.org/onto/prop/google_billing_budget_credit_types">
    <rdfs:label>credit_types</rdfs:label>
    <rdfs:comment>Optional. If creditTypesTreatment is INCLUDE_SPECIFIED_CREDITS,
this is a list of credit types to be subtracted from gross cost to determine the spend for threshold calculations. See a list of acceptable credit type values.
If creditTypesTreatment is not INCLUDE_SPECIFIED_CREDITS, this field must be empty.</rdfs:comment>
    <rdfs:domain rdf:resource="http://example.org/onto/class/google_billing_budget"/>
    <rdfs:range rdf:resource="http://www.w3.org/2001/XMLSchema#string"/>
  </owl:DatatypeProperty>
  <owl:DatatypeProperty rdf:about="http://example.org/onto/prop/google_billing_budget_credit_types_treatment">
    <rdfs:label>credit_types_treatment</rdfs:label>
    <rdfs:comment>Specifies how credits should be treated when determining spend
for threshold calculations. Default value: "INCLUDE_ALL_CREDITS" Possible values: ["INCLUDE_ALL_CREDITS", "EXCLUDE_ALL_CREDITS", "INCLUDE_SPECIFIED_CREDITS"]</rdfs:comment>
    <rdfs:domain rdf:resource="http://example.org/onto/class/google_billing_budget"/>
    <rdfs:range rdf:resource="http://www.w3.org/2001/XMLSchema#string"/>
  </owl:DatatypeProperty>
  <owl:DatatypeProperty rdf:about="http://example.org/onto/prop/google_billing_budget_labels">
    <rdfs:label>labels</rdfs:label>
    <rdfs:comment>A single label and value pair specifying that usage from only
this set of labeled resources should be included in the budget.</rdfs:comment>
    <rdfs:domain rdf:resource="http://example.org/onto/class/google_billing_budget"/>
    <rdfs:range rdf:resource="http://www.w3.org/2001/XMLSchema#string"/>
  </owl:DatatypeProperty>
  <owl:DatatypeProperty rdf:about="http://example.org/onto/prop/google_billing_budget_projects">
    <rdfs:label>projects</rdfs:label>
    <rdfs:comment>A set of projects of the form projects/{project_number},
specifying that usage from only this set of projects should be
included in the budget. If omitted, the report will include
all usage for the billing account, regardless of which project
the usage occurred on.</rdfs:comment>
    <rdfs:domain rdf:resource="http://example.org/onto/class/google_billing_budget"/>
    <rdfs:range rdf:resource="http://www.w3.org/2001/XMLSchema#string"/>
  </owl:DatatypeProperty>
  <owl:DatatypeProperty rdf:about="http://example.org/onto/prop/google_billing_budget_resource_ancestors">
    <rdfs:label>resource_ancestors</rdfs:label>
    <rdfs:comment>A set of folder and organization names of the form folders/{folderId} or organizations/{organizationId},
specifying that usage from only this set of folders and organizations should be included in the budget.
If omitted, the budget includes all usage that the billing account pays for. If the folder or organization
contains projects that are paid for by a different Cloud Billing account, the budget doesn't apply to those projects.</rdfs:comment>
    <rdfs:domain rdf:resource="http://example.org/onto/class/google_billing_budget"/>
    <rdfs:range rdf:resource="http://www.w3.org/2001/XMLSchema#string"/>
  </owl:DatatypeProperty>
  <owl:DatatypeProperty rdf:about="http://example.org/onto/prop/google_billing_budget_services">
    <rdfs:label>services</rdfs:label>
    <rdfs:comment>A set of services of the form services/{service_id},
specifying that usage from only this set of services should be
included in the budget. If omitted, the report will include
usage for all the services. The service names are available
through the Catalog API:
https://cloud.google.com/billing/v1/how-tos/catalog-api.</rdfs:comment>
    <rdfs:domain rdf:resource="http://example.org/onto/class/google_billing_budget"/>
    <rdfs:range rdf:resource="http://www.w3.org/2001/XMLSchema#string"/>
  </owl:DatatypeProperty>
  <owl:DatatypeProperty rdf:about="http://example.org/onto/prop/google_billing_budget_subaccounts">
    <rdfs:label>subaccounts</rdfs:label>
    <rdfs:comment>A set of subaccounts of the form billingAccounts/{account_id},
specifying that usage from only this set of subaccounts should
be included in the budget. If a subaccount is set to the name of
the parent account, usage from the parent account will be included.
If the field is omitted, the report will include usage from the parent
account and all subaccounts, if they exist.</rdfs:comment>
    <rdfs:domain rdf:resource="http://example.org/onto/class/google_billing_budget"/>
    <rdfs:range rdf:resource="http://www.w3.org/2001/XMLSchema#string"/>
  </owl:DatatypeProperty>
  <owl:DatatypeProperty rdf:about="http://example.org/onto/prop/google_billing_budget_day">
    <rdfs:label>day</rdfs:label>
    <rdfs:comment>Day of a month. Must be from 1 to 31 and valid for the year and month.</rdfs:comment>
    <rdfs:domain rdf:resource="http://example.org/onto/class/google_billing_budget"/>
    <rdfs:range rdf:resource="http://www.w3.org/2001/XMLSchema#string"/>
  </owl:DatatypeProperty>
  <owl:DatatypeProperty rdf:about="http://example.org/onto/prop/google_billing_budget_month">
    <rdfs:label>month</rdfs:label>
    <rdfs:comment>Month of a year. Must be from 1 to 12.</rdfs:comment>
    <rdfs:domain rdf:resource="http://example.org/onto/class/google_billing_budget"/>
    <rdfs:range rdf:resource="http://www.w3.org/2001/XMLSchema#string"/>
  </owl:DatatypeProperty>
  <owl:DatatypeProperty rdf:about="http://example.org/onto/prop/google_billing_budget_year">
    <rdfs:label>year</rdfs:label>
    <rdfs:comment>Year of the date. Must be from 1 to 9999.</rdfs:comment>
    <rdfs:domain rdf:resource="http://example.org/onto/class/google_billing_budget"/>
    <rdfs:range rdf:resource="http://www.w3.org/2001/XMLSchema#string"/>
  </owl:DatatypeProperty>
  <owl:DatatypeProperty rdf:about="http://example.org/onto/prop/google_billing_budget_day">
    <rdfs:label>day</rdfs:label>
    <rdfs:comment>Day of a month. Must be from 1 to 31 and valid for the year and month.</rdfs:comment>
    <rdfs:domain rdf:resource="http://example.org/onto/class/google_billing_budget"/>
    <rdfs:range rdf:resource="http://www.w3.org/2001/XMLSchema#string"/>
  </owl:DatatypeProperty>
  <owl:DatatypeProperty rdf:about="http://example.org/onto/prop/google_billing_budget_month">
    <rdfs:label>month</rdfs:label>
    <rdfs:comment>Month of a year. Must be from 1 to 12.</rdfs:comment>
    <rdfs:domain rdf:resource="http://example.org/onto/class/google_billing_budget"/>
    <rdfs:range rdf:resource="http://www.w3.org/2001/XMLSchema#string"/>
  </owl:DatatypeProperty>
  <owl:DatatypeProperty rdf:about="http://example.org/onto/prop/google_billing_budget_year">
    <rdfs:label>year</rdfs:label>
    <rdfs:comment>Year of the date. Must be from 1 to 9999.</rdfs:comment>
    <rdfs:domain rdf:resource="http://example.org/onto/class/google_billing_budget"/>
    <rdfs:range rdf:resource="http://www.w3.org/2001/XMLSchema#string"/>
  </owl:DatatypeProperty>
  <owl:DatatypeProperty rdf:about="http://example.org/onto/prop/google_billing_budget_spend_basis">
    <rdfs:label>spend_basis</rdfs:label>
    <rdfs:comment>The type of basis used to determine if spend has passed
the threshold. Default value: "CURRENT_SPEND" Possible values: ["CURRENT_SPEND", "FORECASTED_SPEND"]</rdfs:comment>
    <rdfs:domain rdf:resource="http://example.org/onto/class/google_billing_budget"/>
    <rdfs:range rdf:resource="http://www.w3.org/2001/XMLSchema#string"/>
  </owl:DatatypeProperty>
  <owl:DatatypeProperty rdf:about="http://example.org/onto/prop/google_billing_budget_threshold_percent">
    <rdfs:label>threshold_percent</rdfs:label>
    <rdfs:comment>Send an alert when this threshold is exceeded. This is a
1.0-based percentage, so 0.5 = 50%. Must be >= 0.</rdfs:comment>
    <rdfs:domain rdf:resource="http://example.org/onto/class/google_billing_budget"/>
    <rdfs:range rdf:resource="http://www.w3.org/2001/XMLSchema#string"/>
  </owl:DatatypeProperty>
  <owl:DatatypeProperty rdf:about="http://example.org/onto/prop/google_billing_budget_create">
    <rdfs:label>create</rdfs:label>
    <rdfs:domain rdf:resource="http://example.org/onto/class/google_billing_budget"/>
    <rdfs:range rdf:resource="http://www.w3.org/2001/XMLSchema#string"/>
  </owl:DatatypeProperty>
  <owl:DatatypeProperty rdf:about="http://example.org/onto/prop/google_billing_budget_delete">
    <rdfs:label>delete</rdfs:label>
    <rdfs:domain rdf:resource="http://example.org/onto/class/google_billing_budget"/>
    <rdfs:range rdf:resource="http://www.w3.org/2001/XMLSchema#string"/>
  </owl:DatatypeProperty>
  <owl:DatatypeProperty rdf:about="http://example.org/onto/prop/google_billing_budget_update">
    <rdfs:label>update</rdfs:label>
    <rdfs:domain rdf:resource="http://example.org/onto/class/google_billing_budget"/>
    <rdfs:range rdf:resource="http://www.w3.org/2001/XMLSchema#string"/>
  </owl:DatatypeProperty>
</rdf:RDF>
