<?xml version="1.0" encoding="UTF-8"?>
<rdf:RDF
  xmlns:rdf="http://www.w3.org/1999/02/22-rdf-syntax-ns#"
  xmlns:rdfs="http://www.w3.org/2000/01/rdf-schema#"
  xmlns:owl="http://www.w3.org/2002/07/owl#"
  xmlns:xsd="http://www.w3.org/2001/XMLSchema#"
  xml:base="http://example.org/onto/">
  <owl:Class rdf:about="http://example.org/onto/class/google_compute_global_address">
    <rdfs:label>google_compute_global_address</rdfs:label>
    <rdfs:comment>#
#     ***     AUTO GENERATED CODE    ***    Type: MMv1     ***
#
# ----------------------------------------------------------------------------
#
#     This code is generated by Magic Modules using the following:
#
#     Configuration: https:#github.com/GoogleCloudPlatform/magic-modules/tree/main/mmv1/products/compute/GlobalAddress.yaml
#     Template:      https:#github.com/GoogleCloudPlatform/magic-modules/tree/main/mmv1/templates/terraform/resource.html.markdown.tmpl
#
#     DO NOT EDIT this file directly. Any changes made to this file will be
#     overwritten during the next generation cycle.
#
# ----------------------------------------------------------------------------
subcategory: "Compute Engine"
description: |-
  Represents a Global Address resource.
---</rdfs:comment>
  </owl:Class>
  <owl:DatatypeProperty rdf:about="http://example.org/onto/prop/google_compute_global_address_address">
    <rdfs:label>address</rdfs:label>
    <rdfs:comment>The IP address or beginning of the address range represented by this
resource. This can be supplied as an input to reserve a specific
address or omitted to allow GCP to choose a valid one for you.</rdfs:comment>
    <rdfs:domain rdf:resource="http://example.org/onto/class/google_compute_global_address"/>
    <rdfs:range rdf:resource="http://www.w3.org/2001/XMLSchema#string"/>
  </owl:DatatypeProperty>
  <owl:DatatypeProperty rdf:about="http://example.org/onto/prop/google_compute_global_address_address_type">
    <rdfs:label>address_type</rdfs:label>
    <rdfs:comment>The type of the address to reserve.

* EXTERNAL indicates public/external single IP address.
* INTERNAL indicates internal IP ranges belonging to some network. Default value: "EXTERNAL" Possible values: ["EXTERNAL", "INTERNAL"]</rdfs:comment>
    <rdfs:domain rdf:resource="http://example.org/onto/class/google_compute_global_address"/>
    <rdfs:range rdf:resource="http://www.w3.org/2001/XMLSchema#string"/>
  </owl:DatatypeProperty>
  <owl:DatatypeProperty rdf:about="http://example.org/onto/prop/google_compute_global_address_creation_timestamp">
    <rdfs:label>creation_timestamp</rdfs:label>
    <rdfs:comment>Creation timestamp in RFC3339 text format.</rdfs:comment>
    <rdfs:domain rdf:resource="http://example.org/onto/class/google_compute_global_address"/>
    <rdfs:range rdf:resource="http://www.w3.org/2001/XMLSchema#string"/>
  </owl:DatatypeProperty>
  <owl:DatatypeProperty rdf:about="http://example.org/onto/prop/google_compute_global_address_description">
    <rdfs:label>description</rdfs:label>
    <rdfs:comment>An optional description of this resource.</rdfs:comment>
    <rdfs:domain rdf:resource="http://example.org/onto/class/google_compute_global_address"/>
    <rdfs:range rdf:resource="http://www.w3.org/2001/XMLSchema#string"/>
  </owl:DatatypeProperty>
  <owl:DatatypeProperty rdf:about="http://example.org/onto/prop/google_compute_global_address_effective_labels">
    <rdfs:label>effective_labels</rdfs:label>
    <rdfs:comment>All of labels (key/value pairs) present on the resource in GCP, including the labels configured through Terraform, other clients and services.</rdfs:comment>
    <rdfs:domain rdf:resource="http://example.org/onto/class/google_compute_global_address"/>
    <rdfs:range rdf:resource="http://www.w3.org/2001/XMLSchema#string"/>
  </owl:DatatypeProperty>
  <owl:DatatypeProperty rdf:about="http://example.org/onto/prop/google_compute_global_address_id">
    <rdfs:label>id</rdfs:label>
    <rdfs:domain rdf:resource="http://example.org/onto/class/google_compute_global_address"/>
    <rdfs:range rdf:resource="http://www.w3.org/2001/XMLSchema#string"/>
  </owl:DatatypeProperty>
  <owl:DatatypeProperty rdf:about="http://example.org/onto/prop/google_compute_global_address_ip_version">
    <rdfs:label>ip_version</rdfs:label>
    <rdfs:comment>The IP Version that will be used by this address. The default value is 'IPV4'. Possible values: ["IPV4", "IPV6"]</rdfs:comment>
    <rdfs:domain rdf:resource="http://example.org/onto/class/google_compute_global_address"/>
    <rdfs:range rdf:resource="http://www.w3.org/2001/XMLSchema#string"/>
  </owl:DatatypeProperty>
  <owl:DatatypeProperty rdf:about="http://example.org/onto/prop/google_compute_global_address_label_fingerprint">
    <rdfs:label>label_fingerprint</rdfs:label>
    <rdfs:comment>The fingerprint used for optimistic locking of this resource.  Used
internally during updates.</rdfs:comment>
    <rdfs:domain rdf:resource="http://example.org/onto/class/google_compute_global_address"/>
    <rdfs:range rdf:resource="http://www.w3.org/2001/XMLSchema#string"/>
  </owl:DatatypeProperty>
  <owl:DatatypeProperty rdf:about="http://example.org/onto/prop/google_compute_global_address_labels">
    <rdfs:label>labels</rdfs:label>
    <rdfs:comment>Labels to apply to this address.  A list of key->value pairs.


**Note**: This field is non-authoritative, and will only manage the labels present in your configuration.
Please refer to the field 'effective_labels' for all of the labels present on the resource.</rdfs:comment>
    <rdfs:domain rdf:resource="http://example.org/onto/class/google_compute_global_address"/>
    <rdfs:range rdf:resource="http://www.w3.org/2001/XMLSchema#string"/>
  </owl:DatatypeProperty>
  <owl:DatatypeProperty rdf:about="http://example.org/onto/prop/google_compute_global_address_name">
    <rdfs:label>name</rdfs:label>
    <rdfs:comment>Name of the resource. Provided by the client when the resource is
created. The name must be 1-63 characters long, and comply with
RFC1035.  Specifically, the name must be 1-63 characters long and
match the regular expression '[a-z]([-a-z0-9]*[a-z0-9])?' which means
the first character must be a lowercase letter, and all following
characters must be a dash, lowercase letter, or digit, except the last
character, which cannot be a dash.</rdfs:comment>
    <rdfs:domain rdf:resource="http://example.org/onto/class/google_compute_global_address"/>
    <rdfs:range rdf:resource="http://www.w3.org/2001/XMLSchema#string"/>
  </owl:DatatypeProperty>
  <owl:DatatypeProperty rdf:about="http://example.org/onto/prop/google_compute_global_address_network">
    <rdfs:label>network</rdfs:label>
    <rdfs:comment>The URL of the network in which to reserve the IP range. The IP range
must be in RFC1918 space. The network cannot be deleted if there are
any reserved IP ranges referring to it.

This should only be set when using an Internal address.</rdfs:comment>
    <rdfs:domain rdf:resource="http://example.org/onto/class/google_compute_global_address"/>
    <rdfs:range rdf:resource="http://www.w3.org/2001/XMLSchema#string"/>
  </owl:DatatypeProperty>
  <owl:DatatypeProperty rdf:about="http://example.org/onto/prop/google_compute_global_address_prefix_length">
    <rdfs:label>prefix_length</rdfs:label>
    <rdfs:comment>The prefix length of the IP range. If not present, it means the
address field is a single IP address.

This field is not applicable to addresses with addressType=INTERNAL
when purpose=PRIVATE_SERVICE_CONNECT</rdfs:comment>
    <rdfs:domain rdf:resource="http://example.org/onto/class/google_compute_global_address"/>
    <rdfs:range rdf:resource="http://www.w3.org/2001/XMLSchema#string"/>
  </owl:DatatypeProperty>
  <owl:DatatypeProperty rdf:about="http://example.org/onto/prop/google_compute_global_address_project">
    <rdfs:label>project</rdfs:label>
    <rdfs:domain rdf:resource="http://example.org/onto/class/google_compute_global_address"/>
    <rdfs:range rdf:resource="http://www.w3.org/2001/XMLSchema#string"/>
  </owl:DatatypeProperty>
  <owl:DatatypeProperty rdf:about="http://example.org/onto/prop/google_compute_global_address_purpose">
    <rdfs:label>purpose</rdfs:label>
    <rdfs:comment>The purpose of the resource. Possible values include:

* VPC_PEERING - for peer networks

* PRIVATE_SERVICE_CONNECT - for ([Beta](https://terraform.io/docs/providers/google/guides/provider_versions.html) only) Private Service Connect networks</rdfs:comment>
    <rdfs:domain rdf:resource="http://example.org/onto/class/google_compute_global_address"/>
    <rdfs:range rdf:resource="http://www.w3.org/2001/XMLSchema#string"/>
  </owl:DatatypeProperty>
  <owl:DatatypeProperty rdf:about="http://example.org/onto/prop/google_compute_global_address_self_link">
    <rdfs:label>self_link</rdfs:label>
    <rdfs:domain rdf:resource="http://example.org/onto/class/google_compute_global_address"/>
    <rdfs:range rdf:resource="http://www.w3.org/2001/XMLSchema#string"/>
  </owl:DatatypeProperty>
  <owl:DatatypeProperty rdf:about="http://example.org/onto/prop/google_compute_global_address_terraform_labels">
    <rdfs:label>terraform_labels</rdfs:label>
    <rdfs:comment>The combination of labels configured directly on the resource
 and default labels configured on the provider.</rdfs:comment>
    <rdfs:domain rdf:resource="http://example.org/onto/class/google_compute_global_address"/>
    <rdfs:range rdf:resource="http://www.w3.org/2001/XMLSchema#string"/>
  </owl:DatatypeProperty>
  <owl:DatatypeProperty rdf:about="http://example.org/onto/prop/google_compute_global_address_create">
    <rdfs:label>create</rdfs:label>
    <rdfs:domain rdf:resource="http://example.org/onto/class/google_compute_global_address"/>
    <rdfs:range rdf:resource="http://www.w3.org/2001/XMLSchema#string"/>
  </owl:DatatypeProperty>
  <owl:DatatypeProperty rdf:about="http://example.org/onto/prop/google_compute_global_address_delete">
    <rdfs:label>delete</rdfs:label>
    <rdfs:domain rdf:resource="http://example.org/onto/class/google_compute_global_address"/>
    <rdfs:range rdf:resource="http://www.w3.org/2001/XMLSchema#string"/>
  </owl:DatatypeProperty>
  <owl:DatatypeProperty rdf:about="http://example.org/onto/prop/google_compute_global_address_update">
    <rdfs:label>update</rdfs:label>
    <rdfs:domain rdf:resource="http://example.org/onto/class/google_compute_global_address"/>
    <rdfs:range rdf:resource="http://www.w3.org/2001/XMLSchema#string"/>
  </owl:DatatypeProperty>
</rdf:RDF>
