<?xml version="1.0" encoding="UTF-8"?>
<rdf:RDF
  xmlns:rdf="http://www.w3.org/1999/02/22-rdf-syntax-ns#"
  xmlns:rdfs="http://www.w3.org/2000/01/rdf-schema#"
  xmlns:owl="http://www.w3.org/2002/07/owl#"
  xmlns:xsd="http://www.w3.org/2001/XMLSchema#"
  xml:base="http://example.org/onto/">
  <owl:Class rdf:about="http://example.org/onto/class/google_iam_workforce_pool_provider">
    <rdfs:label>google_iam_workforce_pool_provider</rdfs:label>
    <rdfs:comment>#
#     ***     AUTO GENERATED CODE    ***    Type: MMv1     ***
#
# ----------------------------------------------------------------------------
#
#     This code is generated by Magic Modules using the following:
#
#     Configuration: https:#github.com/GoogleCloudPlatform/magic-modules/tree/main/mmv1/products/iamworkforcepool/WorkforcePoolProvider.yaml
#     Template:      https:#github.com/GoogleCloudPlatform/magic-modules/tree/main/mmv1/templates/terraform/resource.html.markdown.tmpl
#
#     DO NOT EDIT this file directly. Any changes made to this file will be
#     overwritten during the next generation cycle.
#
# ----------------------------------------------------------------------------
subcategory: "Cloud IAM"
description: |-
  A configuration for an external identity provider.
---</rdfs:comment>
  </owl:Class>
  <owl:DatatypeProperty rdf:about="http://example.org/onto/prop/google_iam_workforce_pool_provider_attribute_condition">
    <rdfs:label>attribute_condition</rdfs:label>
    <rdfs:comment>A [Common Expression Language](https://opensource.google/projects/cel) expression, in
plain text, to restrict what otherwise valid authentication credentials issued by the
provider should not be accepted.

The expression must output a boolean representing whether to allow the federation.

The following keywords may be referenced in the expressions:
  * 'assertion': JSON representing the authentication credential issued by the provider.
  * 'google': The Google attributes mapped from the assertion in the 'attribute_mappings'.
    'google.profile_photo' and 'google.display_name' are not supported.
  * 'attribute': The custom attributes mapped from the assertion in the 'attribute_mappings'.

The maximum length of the attribute condition expression is 4096 characters.
If unspecified, all valid authentication credentials will be accepted.

The following example shows how to only allow credentials with a mapped 'google.groups' value of 'admins':
'''
"'admins' in google.groups"
'''</rdfs:comment>
    <rdfs:domain rdf:resource="http://example.org/onto/class/google_iam_workforce_pool_provider"/>
    <rdfs:range rdf:resource="http://www.w3.org/2001/XMLSchema#string"/>
  </owl:DatatypeProperty>
  <owl:DatatypeProperty rdf:about="http://example.org/onto/prop/google_iam_workforce_pool_provider_attribute_mapping">
    <rdfs:label>attribute_mapping</rdfs:label>
    <rdfs:comment>Maps attributes from the authentication credentials issued by an external identity provider
to Google Cloud attributes, such as 'subject' and 'segment'.

Each key must be a string specifying the Google Cloud IAM attribute to map to.

The following keys are supported:
  * 'google.subject': The principal IAM is authenticating. You can reference this value in IAM bindings.
    This is also the subject that appears in Cloud Logging logs. This is a required field and
    the mapped subject cannot exceed 127 bytes.
  * 'google.groups': Groups the authenticating user belongs to. You can grant groups access to
    resources using an IAM 'principalSet' binding; access applies to all members of the group.
  * 'google.display_name': The name of the authenticated user. This is an optional field and
    the mapped display name cannot exceed 100 bytes. If not set, 'google.subject' will be displayed instead.
    This attribute cannot be referenced in IAM bindings.
  * 'google.profile_photo': The URL that specifies the authenticated user's thumbnail photo.
    This is an optional field. When set, the image will be visible as the user's profile picture.
    If not set, a generic user icon will be displayed instead.
    This attribute cannot be referenced in IAM bindings.

You can also provide custom attributes by specifying 'attribute.{custom_attribute}', where {custom_attribute}
is the name of the custom attribute to be mapped. You can define a maximum of 50 custom attributes.
The maximum length of a mapped attribute key is 100 characters, and the key may only contain the characters [a-z0-9_].

You can reference these attributes in IAM policies to define fine-grained access for a workforce pool
to Google Cloud resources. For example:
  * 'google.subject':
    'principal://iam.googleapis.com/locations/{location}/workforcePools/{pool}/subject/{value}'
  * 'google.groups':
    'principalSet://iam.googleapis.com/locations/{location}/workforcePools/{pool}/group/{value}'
  * 'attribute.{custom_attribute}':
    'principalSet://iam.googleapis.com/locations/{location}/workforcePools/{pool}/attribute.{custom_attribute}/{value}'

Each value must be a [Common Expression Language](https://opensource.google/projects/cel)
function that maps an identity provider credential to the normalized attribute specified
by the corresponding map key.

You can use the 'assertion' keyword in the expression to access a JSON representation of
the authentication credential issued by the provider.

The maximum length of an attribute mapping expression is 2048 characters. When evaluated,
the total size of all mapped attributes must not exceed 8KB.

For OIDC providers, you must supply a custom mapping that includes the 'google.subject' attribute.
For example, the following maps the sub claim of the incoming credential to the 'subject' attribute
on a Google token:
'''
{"google.subject": "assertion.sub"}
'''

An object containing a list of '"key": value' pairs.
Example: '{ "name": "wrench", "mass": "1.3kg", "count": "3" }'.</rdfs:comment>
    <rdfs:domain rdf:resource="http://example.org/onto/class/google_iam_workforce_pool_provider"/>
    <rdfs:range rdf:resource="http://www.w3.org/2001/XMLSchema#string"/>
  </owl:DatatypeProperty>
  <owl:DatatypeProperty rdf:about="http://example.org/onto/prop/google_iam_workforce_pool_provider_description">
    <rdfs:label>description</rdfs:label>
    <rdfs:comment>A user-specified description of the provider. Cannot exceed 256 characters.</rdfs:comment>
    <rdfs:domain rdf:resource="http://example.org/onto/class/google_iam_workforce_pool_provider"/>
    <rdfs:range rdf:resource="http://www.w3.org/2001/XMLSchema#string"/>
  </owl:DatatypeProperty>
  <owl:DatatypeProperty rdf:about="http://example.org/onto/prop/google_iam_workforce_pool_provider_disabled">
    <rdfs:label>disabled</rdfs:label>
    <rdfs:comment>Whether the provider is disabled. You cannot use a disabled provider to exchange tokens.
However, existing tokens still grant access.</rdfs:comment>
    <rdfs:domain rdf:resource="http://example.org/onto/class/google_iam_workforce_pool_provider"/>
    <rdfs:range rdf:resource="http://www.w3.org/2001/XMLSchema#string"/>
  </owl:DatatypeProperty>
  <owl:DatatypeProperty rdf:about="http://example.org/onto/prop/google_iam_workforce_pool_provider_display_name">
    <rdfs:label>display_name</rdfs:label>
    <rdfs:comment>A user-specified display name for the provider. Cannot exceed 32 characters.</rdfs:comment>
    <rdfs:domain rdf:resource="http://example.org/onto/class/google_iam_workforce_pool_provider"/>
    <rdfs:range rdf:resource="http://www.w3.org/2001/XMLSchema#string"/>
  </owl:DatatypeProperty>
  <owl:DatatypeProperty rdf:about="http://example.org/onto/prop/google_iam_workforce_pool_provider_id">
    <rdfs:label>id</rdfs:label>
    <rdfs:domain rdf:resource="http://example.org/onto/class/google_iam_workforce_pool_provider"/>
    <rdfs:range rdf:resource="http://www.w3.org/2001/XMLSchema#string"/>
  </owl:DatatypeProperty>
  <owl:DatatypeProperty rdf:about="http://example.org/onto/prop/google_iam_workforce_pool_provider_location">
    <rdfs:label>location</rdfs:label>
    <rdfs:comment>The location for the resource.</rdfs:comment>
    <rdfs:domain rdf:resource="http://example.org/onto/class/google_iam_workforce_pool_provider"/>
    <rdfs:range rdf:resource="http://www.w3.org/2001/XMLSchema#string"/>
  </owl:DatatypeProperty>
  <owl:DatatypeProperty rdf:about="http://example.org/onto/prop/google_iam_workforce_pool_provider_name">
    <rdfs:label>name</rdfs:label>
    <rdfs:comment>Output only. The resource name of the provider.
Format: 'locations/{location}/workforcePools/{workforcePoolId}/providers/{providerId}'</rdfs:comment>
    <rdfs:domain rdf:resource="http://example.org/onto/class/google_iam_workforce_pool_provider"/>
    <rdfs:range rdf:resource="http://www.w3.org/2001/XMLSchema#string"/>
  </owl:DatatypeProperty>
  <owl:DatatypeProperty rdf:about="http://example.org/onto/prop/google_iam_workforce_pool_provider_provider_id">
    <rdfs:label>provider_id</rdfs:label>
    <rdfs:comment>The ID for the provider, which becomes the final component of the resource name.
This value must be 4-32 characters, and may contain the characters [a-z0-9-].
The prefix 'gcp-' is reserved for use by Google, and may not be specified.</rdfs:comment>
    <rdfs:domain rdf:resource="http://example.org/onto/class/google_iam_workforce_pool_provider"/>
    <rdfs:range rdf:resource="http://www.w3.org/2001/XMLSchema#string"/>
  </owl:DatatypeProperty>
  <owl:DatatypeProperty rdf:about="http://example.org/onto/prop/google_iam_workforce_pool_provider_state">
    <rdfs:label>state</rdfs:label>
    <rdfs:comment>The current state of the provider.
* STATE_UNSPECIFIED: State unspecified.
* ACTIVE: The provider is active and may be used to validate authentication credentials.
* DELETED: The provider is soft-deleted. Soft-deleted providers are permanently
  deleted after approximately 30 days. You can restore a soft-deleted provider using
  [providers.undelete](https://cloud.google.com/iam/docs/reference/rest/v1/locations.workforcePools.providers/undelete#google.iam.admin.v1.WorkforcePools.UndeleteWorkforcePoolProvider).</rdfs:comment>
    <rdfs:domain rdf:resource="http://example.org/onto/class/google_iam_workforce_pool_provider"/>
    <rdfs:range rdf:resource="http://www.w3.org/2001/XMLSchema#string"/>
  </owl:DatatypeProperty>
  <owl:DatatypeProperty rdf:about="http://example.org/onto/prop/google_iam_workforce_pool_provider_workforce_pool_id">
    <rdfs:label>workforce_pool_id</rdfs:label>
    <rdfs:comment>The ID to use for the pool, which becomes the final component of the resource name.
The IDs must be a globally unique string of 6 to 63 lowercase letters, digits, or hyphens.
It must start with a letter, and cannot have a trailing hyphen.
The prefix 'gcp-' is reserved for use by Google, and may not be specified.</rdfs:comment>
    <rdfs:domain rdf:resource="http://example.org/onto/class/google_iam_workforce_pool_provider"/>
    <rdfs:range rdf:resource="http://www.w3.org/2001/XMLSchema#string"/>
  </owl:DatatypeProperty>
  <owl:DatatypeProperty rdf:about="http://example.org/onto/prop/google_iam_workforce_pool_provider_attributes_type">
    <rdfs:label>attributes_type</rdfs:label>
    <rdfs:comment>Represents the IdP and type of claims that should be fetched.
* AZURE_AD_GROUPS_ID:  Used to get the user's group claims from the Azure AD identity provider
using configuration provided in ExtendedAttributesOAuth2Client and 'id'
property of the 'microsoft.graph.group' object is used for claim mapping. See
https://learn.microsoft.com/en-us/graph/api/resources/group?view=graph-rest-1.0#properties
for more details on 'microsoft.graph.group' properties. The
group IDs obtained from Azure AD are present in 'assertion.groups' for
OIDC providers and 'assertion.attributes.groups' for SAML providers for
attribute mapping. Possible values: ["AZURE_AD_GROUPS_ID"]</rdfs:comment>
    <rdfs:domain rdf:resource="http://example.org/onto/class/google_iam_workforce_pool_provider"/>
    <rdfs:range rdf:resource="http://www.w3.org/2001/XMLSchema#string"/>
  </owl:DatatypeProperty>
  <owl:DatatypeProperty rdf:about="http://example.org/onto/prop/google_iam_workforce_pool_provider_client_id">
    <rdfs:label>client_id</rdfs:label>
    <rdfs:comment>The OAuth 2.0 client ID for retrieving extended attributes from the identity provider. Required to get the Access Token using client credentials grant flow.</rdfs:comment>
    <rdfs:domain rdf:resource="http://example.org/onto/class/google_iam_workforce_pool_provider"/>
    <rdfs:range rdf:resource="http://www.w3.org/2001/XMLSchema#string"/>
  </owl:DatatypeProperty>
  <owl:DatatypeProperty rdf:about="http://example.org/onto/prop/google_iam_workforce_pool_provider_issuer_uri">
    <rdfs:label>issuer_uri</rdfs:label>
    <rdfs:comment>The OIDC identity provider's issuer URI. Must be a valid URI using the 'https' scheme. Required to get the OIDC discovery document.</rdfs:comment>
    <rdfs:domain rdf:resource="http://example.org/onto/class/google_iam_workforce_pool_provider"/>
    <rdfs:range rdf:resource="http://www.w3.org/2001/XMLSchema#string"/>
  </owl:DatatypeProperty>
  <owl:DatatypeProperty rdf:about="http://example.org/onto/prop/google_iam_workforce_pool_provider_plain_text">
    <rdfs:label>plain_text</rdfs:label>
    <rdfs:comment>The plain text of the client secret value.</rdfs:comment>
    <rdfs:domain rdf:resource="http://example.org/onto/class/google_iam_workforce_pool_provider"/>
    <rdfs:range rdf:resource="http://www.w3.org/2001/XMLSchema#string"/>
  </owl:DatatypeProperty>
  <owl:DatatypeProperty rdf:about="http://example.org/onto/prop/google_iam_workforce_pool_provider_thumbprint">
    <rdfs:label>thumbprint</rdfs:label>
    <rdfs:comment>A thumbprint to represent the current client secret value.</rdfs:comment>
    <rdfs:domain rdf:resource="http://example.org/onto/class/google_iam_workforce_pool_provider"/>
    <rdfs:range rdf:resource="http://www.w3.org/2001/XMLSchema#string"/>
  </owl:DatatypeProperty>
  <owl:DatatypeProperty rdf:about="http://example.org/onto/prop/google_iam_workforce_pool_provider_filter">
    <rdfs:label>filter</rdfs:label>
    <rdfs:comment>The filter used to request specific records from IdP. In case of attributes type as AZURE_AD_GROUPS_ID, it represents the
filter used to request specific groups for users from IdP. By default, all of the groups associated with the user are fetched. The
groups should be security enabled. See https://learn.microsoft.com/en-us/graph/search-query-parameter for more details.</rdfs:comment>
    <rdfs:domain rdf:resource="http://example.org/onto/class/google_iam_workforce_pool_provider"/>
    <rdfs:range rdf:resource="http://www.w3.org/2001/XMLSchema#string"/>
  </owl:DatatypeProperty>
  <owl:DatatypeProperty rdf:about="http://example.org/onto/prop/google_iam_workforce_pool_provider_attributes_type">
    <rdfs:label>attributes_type</rdfs:label>
    <rdfs:comment>Represents the IdP and type of claims that should be fetched.
* AZURE_AD_GROUPS_MAIL: Used to get the user's group claims from the Azure AD identity provider using configuration provided
in ExtraAttributesOAuth2Client and 'mail' property of the 'microsoft.graph.group' object is used for claim mapping.
See https://learn.microsoft.com/en-us/graph/api/resources/group?view=graph-rest-1.0#properties for more details on
'microsoft.graph.group' properties. The attributes obtained from idntity provider are mapped to 'assertion.groups'.
* AZURE_AD_GROUPS_ID:  Used to get the user's group claims from the Azure AD identity provider
using configuration provided in ExtraAttributesOAuth2Client and 'id'
property of the 'microsoft.graph.group' object is used for claim mapping. See
https://learn.microsoft.com/en-us/graph/api/resources/group?view=graph-rest-1.0#properties
for more details on 'microsoft.graph.group' properties. The
group IDs obtained from Azure AD are present in 'assertion.groups' for
OIDC providers and 'assertion.attributes.groups' for SAML providers for
attribute mapping. Possible values: ["AZURE_AD_GROUPS_MAIL", "AZURE_AD_GROUPS_ID"]</rdfs:comment>
    <rdfs:domain rdf:resource="http://example.org/onto/class/google_iam_workforce_pool_provider"/>
    <rdfs:range rdf:resource="http://www.w3.org/2001/XMLSchema#string"/>
  </owl:DatatypeProperty>
  <owl:DatatypeProperty rdf:about="http://example.org/onto/prop/google_iam_workforce_pool_provider_client_id">
    <rdfs:label>client_id</rdfs:label>
    <rdfs:comment>The OAuth 2.0 client ID for retrieving extra attributes from the identity provider. Required to get the Access Token using client credentials grant flow.</rdfs:comment>
    <rdfs:domain rdf:resource="http://example.org/onto/class/google_iam_workforce_pool_provider"/>
    <rdfs:range rdf:resource="http://www.w3.org/2001/XMLSchema#string"/>
  </owl:DatatypeProperty>
  <owl:DatatypeProperty rdf:about="http://example.org/onto/prop/google_iam_workforce_pool_provider_issuer_uri">
    <rdfs:label>issuer_uri</rdfs:label>
    <rdfs:comment>The OIDC identity provider's issuer URI. Must be a valid URI using the 'https' scheme. Required to get the OIDC discovery document.</rdfs:comment>
    <rdfs:domain rdf:resource="http://example.org/onto/class/google_iam_workforce_pool_provider"/>
    <rdfs:range rdf:resource="http://www.w3.org/2001/XMLSchema#string"/>
  </owl:DatatypeProperty>
  <owl:DatatypeProperty rdf:about="http://example.org/onto/prop/google_iam_workforce_pool_provider_plain_text">
    <rdfs:label>plain_text</rdfs:label>
    <rdfs:comment>The plain text of the client secret value.</rdfs:comment>
    <rdfs:domain rdf:resource="http://example.org/onto/class/google_iam_workforce_pool_provider"/>
    <rdfs:range rdf:resource="http://www.w3.org/2001/XMLSchema#string"/>
  </owl:DatatypeProperty>
  <owl:DatatypeProperty rdf:about="http://example.org/onto/prop/google_iam_workforce_pool_provider_thumbprint">
    <rdfs:label>thumbprint</rdfs:label>
    <rdfs:comment>A thumbprint to represent the current client secret value.</rdfs:comment>
    <rdfs:domain rdf:resource="http://example.org/onto/class/google_iam_workforce_pool_provider"/>
    <rdfs:range rdf:resource="http://www.w3.org/2001/XMLSchema#string"/>
  </owl:DatatypeProperty>
  <owl:DatatypeProperty rdf:about="http://example.org/onto/prop/google_iam_workforce_pool_provider_filter">
    <rdfs:label>filter</rdfs:label>
    <rdfs:comment>The filter used to request specific records from IdP. In case of attributes type as AZURE_AD_GROUPS_MAIL and AZURE_AD_GROUPS_ID, it represents the
filter used to request specific groups for users from IdP. By default, all of the groups associated with the user are fetched. The
groups should be security enabled. See https://learn.microsoft.com/en-us/graph/search-query-parameter for more details.</rdfs:comment>
    <rdfs:domain rdf:resource="http://example.org/onto/class/google_iam_workforce_pool_provider"/>
    <rdfs:range rdf:resource="http://www.w3.org/2001/XMLSchema#string"/>
  </owl:DatatypeProperty>
  <owl:DatatypeProperty rdf:about="http://example.org/onto/prop/google_iam_workforce_pool_provider_client_id">
    <rdfs:label>client_id</rdfs:label>
    <rdfs:comment>The client ID. Must match the audience claim of the JWT issued by the identity provider.</rdfs:comment>
    <rdfs:domain rdf:resource="http://example.org/onto/class/google_iam_workforce_pool_provider"/>
    <rdfs:range rdf:resource="http://www.w3.org/2001/XMLSchema#string"/>
  </owl:DatatypeProperty>
  <owl:DatatypeProperty rdf:about="http://example.org/onto/prop/google_iam_workforce_pool_provider_issuer_uri">
    <rdfs:label>issuer_uri</rdfs:label>
    <rdfs:comment>The OIDC issuer URI. Must be a valid URI using the 'https' scheme.</rdfs:comment>
    <rdfs:domain rdf:resource="http://example.org/onto/class/google_iam_workforce_pool_provider"/>
    <rdfs:range rdf:resource="http://www.w3.org/2001/XMLSchema#string"/>
  </owl:DatatypeProperty>
  <owl:DatatypeProperty rdf:about="http://example.org/onto/prop/google_iam_workforce_pool_provider_jwks_json">
    <rdfs:label>jwks_json</rdfs:label>
    <rdfs:comment>OIDC JWKs in JSON String format. For details on definition of a
JWK, see https:tools.ietf.org/html/rfc7517. If not set, then we
use the 'jwks_uri' from the discovery document fetched from the
.well-known path for the 'issuer_uri'. Currently, RSA and EC asymmetric
keys are supported. The JWK must use following format and include only
the following fields:
'''
{
  "keys": [
    {
          "kty": "RSA/EC",
          "alg": "<algorithm>",
          "use": "sig",
          "kid": "<key-id>",
          "n": "",
          "e": "",
          "x": "",
          "y": "",
          "crv": ""
    }
  ]
}
'''</rdfs:comment>
    <rdfs:domain rdf:resource="http://example.org/onto/class/google_iam_workforce_pool_provider"/>
    <rdfs:range rdf:resource="http://www.w3.org/2001/XMLSchema#string"/>
  </owl:DatatypeProperty>
  <owl:DatatypeProperty rdf:about="http://example.org/onto/prop/google_iam_workforce_pool_provider_plain_text">
    <rdfs:label>plain_text</rdfs:label>
    <rdfs:comment>The plain text of the client secret value.</rdfs:comment>
    <rdfs:domain rdf:resource="http://example.org/onto/class/google_iam_workforce_pool_provider"/>
    <rdfs:range rdf:resource="http://www.w3.org/2001/XMLSchema#string"/>
  </owl:DatatypeProperty>
  <owl:DatatypeProperty rdf:about="http://example.org/onto/prop/google_iam_workforce_pool_provider_thumbprint">
    <rdfs:label>thumbprint</rdfs:label>
    <rdfs:comment>A thumbprint to represent the current client secret value.</rdfs:comment>
    <rdfs:domain rdf:resource="http://example.org/onto/class/google_iam_workforce_pool_provider"/>
    <rdfs:range rdf:resource="http://www.w3.org/2001/XMLSchema#string"/>
  </owl:DatatypeProperty>
  <owl:DatatypeProperty rdf:about="http://example.org/onto/prop/google_iam_workforce_pool_provider_additional_scopes">
    <rdfs:label>additional_scopes</rdfs:label>
    <rdfs:comment>Additional scopes to request for in the OIDC authentication request on top of scopes requested by default. By default, the 'openid', 'profile' and 'email' scopes that are supported by the identity provider are requested.
Each additional scope may be at most 256 characters. A maximum of 10 additional scopes may be configured.</rdfs:comment>
    <rdfs:domain rdf:resource="http://example.org/onto/class/google_iam_workforce_pool_provider"/>
    <rdfs:range rdf:resource="http://www.w3.org/2001/XMLSchema#string"/>
  </owl:DatatypeProperty>
  <owl:DatatypeProperty rdf:about="http://example.org/onto/prop/google_iam_workforce_pool_provider_assertion_claims_behavior">
    <rdfs:label>assertion_claims_behavior</rdfs:label>
    <rdfs:comment>The behavior for how OIDC Claims are included in the 'assertion' object used for attribute mapping and attribute condition.
* MERGE_USER_INFO_OVER_ID_TOKEN_CLAIMS: Merge the UserInfo Endpoint Claims with ID Token Claims, preferring UserInfo Claim Values for the same Claim Name. This option is available only for the Authorization Code Flow.
* ONLY_ID_TOKEN_CLAIMS: Only include ID Token Claims. Possible values: ["MERGE_USER_INFO_OVER_ID_TOKEN_CLAIMS", "ONLY_ID_TOKEN_CLAIMS"]</rdfs:comment>
    <rdfs:domain rdf:resource="http://example.org/onto/class/google_iam_workforce_pool_provider"/>
    <rdfs:range rdf:resource="http://www.w3.org/2001/XMLSchema#string"/>
  </owl:DatatypeProperty>
  <owl:DatatypeProperty rdf:about="http://example.org/onto/prop/google_iam_workforce_pool_provider_response_type">
    <rdfs:label>response_type</rdfs:label>
    <rdfs:comment>The Response Type to request for in the OIDC Authorization Request for web sign-in.

The 'CODE' Response Type is recommended to avoid the Implicit Flow, for security reasons.
* CODE: The 'response_type=code' selection uses the Authorization Code Flow for web sign-in. Requires a configured client secret.
* ID_TOKEN: The 'response_type=id_token' selection uses the Implicit Flow for web sign-in. Possible values: ["CODE", "ID_TOKEN"]</rdfs:comment>
    <rdfs:domain rdf:resource="http://example.org/onto/class/google_iam_workforce_pool_provider"/>
    <rdfs:range rdf:resource="http://www.w3.org/2001/XMLSchema#string"/>
  </owl:DatatypeProperty>
  <owl:DatatypeProperty rdf:about="http://example.org/onto/prop/google_iam_workforce_pool_provider_idp_metadata_xml">
    <rdfs:label>idp_metadata_xml</rdfs:label>
    <rdfs:comment>SAML Identity provider configuration metadata xml doc.
The xml document should comply with [SAML 2.0 specification](https://docs.oasis-open.org/security/saml/v2.0/saml-metadata-2.0-os.pdf).
The max size of the acceptable xml document will be bounded to 128k characters.

The metadata xml document should satisfy the following constraints:
1) Must contain an Identity Provider Entity ID.
2) Must contain at least one non-expired signing key certificate.
3) For each signing key:
  a) Valid from should be no more than 7 days from now.
  b) Valid to should be no more than 10 years in the future.
4) Up to 3 IdP signing keys are allowed in the metadata xml.

When updating the provider's metadata xml, at least one non-expired signing key
must overlap with the existing metadata. This requirement is skipped if there are
no non-expired signing keys present in the existing metadata.</rdfs:comment>
    <rdfs:domain rdf:resource="http://example.org/onto/class/google_iam_workforce_pool_provider"/>
    <rdfs:range rdf:resource="http://www.w3.org/2001/XMLSchema#string"/>
  </owl:DatatypeProperty>
  <owl:DatatypeProperty rdf:about="http://example.org/onto/prop/google_iam_workforce_pool_provider_create">
    <rdfs:label>create</rdfs:label>
    <rdfs:domain rdf:resource="http://example.org/onto/class/google_iam_workforce_pool_provider"/>
    <rdfs:range rdf:resource="http://www.w3.org/2001/XMLSchema#string"/>
  </owl:DatatypeProperty>
  <owl:DatatypeProperty rdf:about="http://example.org/onto/prop/google_iam_workforce_pool_provider_delete">
    <rdfs:label>delete</rdfs:label>
    <rdfs:domain rdf:resource="http://example.org/onto/class/google_iam_workforce_pool_provider"/>
    <rdfs:range rdf:resource="http://www.w3.org/2001/XMLSchema#string"/>
  </owl:DatatypeProperty>
  <owl:DatatypeProperty rdf:about="http://example.org/onto/prop/google_iam_workforce_pool_provider_update">
    <rdfs:label>update</rdfs:label>
    <rdfs:domain rdf:resource="http://example.org/onto/class/google_iam_workforce_pool_provider"/>
    <rdfs:range rdf:resource="http://www.w3.org/2001/XMLSchema#string"/>
  </owl:DatatypeProperty>
</rdf:RDF>
