<?xml version="1.0" encoding="UTF-8"?>
<rdf:RDF
  xmlns:rdf="http://www.w3.org/1999/02/22-rdf-syntax-ns#"
  xmlns:rdfs="http://www.w3.org/2000/01/rdf-schema#"
  xmlns:owl="http://www.w3.org/2002/07/owl#"
  xmlns:xsd="http://www.w3.org/2001/XMLSchema#"
  xml:base="http://example.org/onto/">
  <owl:Class rdf:about="http://example.org/onto/class/google_managed_kafka_acl">
    <rdfs:label>google_managed_kafka_acl</rdfs:label>
    <rdfs:comment>#
#     ***     AUTO GENERATED CODE    ***    Type: MMv1     ***
#
# ----------------------------------------------------------------------------
#
#     This code is generated by Magic Modules using the following:
#
#     Configuration: https:#github.com/GoogleCloudPlatform/magic-modules/tree/main/mmv1/products/managedkafka/Acl.yaml
#     Template:      https:#github.com/GoogleCloudPlatform/magic-modules/tree/main/mmv1/templates/terraform/resource.html.markdown.tmpl
#
#     DO NOT EDIT this file directly. Any changes made to this file will be
#     overwritten during the next generation cycle.
#
# ----------------------------------------------------------------------------
subcategory: "Managed Kafka"
description: |-
  A Managed Service for Apache Kafka ACL.
---</rdfs:comment>
  </owl:Class>
  <owl:DatatypeProperty rdf:about="http://example.org/onto/prop/google_managed_kafka_acl_acl_id">
    <rdfs:label>acl_id</rdfs:label>
    <rdfs:comment>The ID to use for the acl, which will become the final component of the acl's name. The structure of 'aclId' defines the Resource Pattern (resource_type, resource_name, pattern_type) of the acl. 'aclId' is structured like one of the following:
For acls on the cluster: 'cluster'
For acls on a single resource within the cluster: 'topic/{resource_name}' 'consumerGroup/{resource_name}' 'transactionalId/{resource_name}'
For acls on all resources that match a prefix: 'topicPrefixed/{resource_name}' 'consumerGroupPrefixed/{resource_name}' 'transactionalIdPrefixed/{resource_name}'
For acls on all resources of a given type (i.e. the wildcard literal '*''): 'allTopics' (represents 'topic/*') 'allConsumerGroups' (represents 'consumerGroup/*') 'allTransactionalIds' (represents 'transactionalId/*').</rdfs:comment>
    <rdfs:domain rdf:resource="http://example.org/onto/class/google_managed_kafka_acl"/>
    <rdfs:range rdf:resource="http://www.w3.org/2001/XMLSchema#string"/>
  </owl:DatatypeProperty>
  <owl:DatatypeProperty rdf:about="http://example.org/onto/prop/google_managed_kafka_acl_cluster">
    <rdfs:label>cluster</rdfs:label>
    <rdfs:comment>The cluster name.</rdfs:comment>
    <rdfs:domain rdf:resource="http://example.org/onto/class/google_managed_kafka_acl"/>
    <rdfs:range rdf:resource="http://www.w3.org/2001/XMLSchema#string"/>
  </owl:DatatypeProperty>
  <owl:DatatypeProperty rdf:about="http://example.org/onto/prop/google_managed_kafka_acl_etag">
    <rdfs:label>etag</rdfs:label>
    <rdfs:comment>'etag' is used for concurrency control. An 'etag' is returned in the
response to 'GetAcl' and 'CreateAcl'. Callers are required to put that etag
in the request to 'UpdateAcl' to ensure that their change will be applied
to the same version of the acl that exists in the Kafka Cluster.

A terminal 'T' character in the etag indicates that the AclEntries were
truncated due to repeated field limits.</rdfs:comment>
    <rdfs:domain rdf:resource="http://example.org/onto/class/google_managed_kafka_acl"/>
    <rdfs:range rdf:resource="http://www.w3.org/2001/XMLSchema#string"/>
  </owl:DatatypeProperty>
  <owl:DatatypeProperty rdf:about="http://example.org/onto/prop/google_managed_kafka_acl_id">
    <rdfs:label>id</rdfs:label>
    <rdfs:domain rdf:resource="http://example.org/onto/class/google_managed_kafka_acl"/>
    <rdfs:range rdf:resource="http://www.w3.org/2001/XMLSchema#string"/>
  </owl:DatatypeProperty>
  <owl:DatatypeProperty rdf:about="http://example.org/onto/prop/google_managed_kafka_acl_location">
    <rdfs:label>location</rdfs:label>
    <rdfs:comment>ID of the location of the Kafka resource. See https://cloud.google.com/managed-kafka/docs/locations for a list of supported locations.</rdfs:comment>
    <rdfs:domain rdf:resource="http://example.org/onto/class/google_managed_kafka_acl"/>
    <rdfs:range rdf:resource="http://www.w3.org/2001/XMLSchema#string"/>
  </owl:DatatypeProperty>
  <owl:DatatypeProperty rdf:about="http://example.org/onto/prop/google_managed_kafka_acl_name">
    <rdfs:label>name</rdfs:label>
    <rdfs:comment>The name of the acl. The 'ACL_ID' segment is used when connecting directly to the cluster. Must be in the format 'projects/PROJECT_ID/locations/LOCATION/clusters/CLUSTER_ID/acls/ACL_ID'.</rdfs:comment>
    <rdfs:domain rdf:resource="http://example.org/onto/class/google_managed_kafka_acl"/>
    <rdfs:range rdf:resource="http://www.w3.org/2001/XMLSchema#string"/>
  </owl:DatatypeProperty>
  <owl:DatatypeProperty rdf:about="http://example.org/onto/prop/google_managed_kafka_acl_pattern_type">
    <rdfs:label>pattern_type</rdfs:label>
    <rdfs:comment>The acl pattern type derived from the name. One of: LITERAL, PREFIXED.</rdfs:comment>
    <rdfs:domain rdf:resource="http://example.org/onto/class/google_managed_kafka_acl"/>
    <rdfs:range rdf:resource="http://www.w3.org/2001/XMLSchema#string"/>
  </owl:DatatypeProperty>
  <owl:DatatypeProperty rdf:about="http://example.org/onto/prop/google_managed_kafka_acl_project">
    <rdfs:label>project</rdfs:label>
    <rdfs:domain rdf:resource="http://example.org/onto/class/google_managed_kafka_acl"/>
    <rdfs:range rdf:resource="http://www.w3.org/2001/XMLSchema#string"/>
  </owl:DatatypeProperty>
  <owl:DatatypeProperty rdf:about="http://example.org/onto/prop/google_managed_kafka_acl_resource_name">
    <rdfs:label>resource_name</rdfs:label>
    <rdfs:comment>The acl resource name derived from the name. For cluster resource_type, this is always "kafka-cluster". Can be the wildcard literal "*".</rdfs:comment>
    <rdfs:domain rdf:resource="http://example.org/onto/class/google_managed_kafka_acl"/>
    <rdfs:range rdf:resource="http://www.w3.org/2001/XMLSchema#string"/>
  </owl:DatatypeProperty>
  <owl:DatatypeProperty rdf:about="http://example.org/onto/prop/google_managed_kafka_acl_resource_type">
    <rdfs:label>resource_type</rdfs:label>
    <rdfs:comment>The acl resource type derived from the name. One of: CLUSTER, TOPIC, GROUP, TRANSACTIONAL_ID.</rdfs:comment>
    <rdfs:domain rdf:resource="http://example.org/onto/class/google_managed_kafka_acl"/>
    <rdfs:range rdf:resource="http://www.w3.org/2001/XMLSchema#string"/>
  </owl:DatatypeProperty>
  <owl:DatatypeProperty rdf:about="http://example.org/onto/prop/google_managed_kafka_acl_host">
    <rdfs:label>host</rdfs:label>
    <rdfs:comment>The host. Must be set to "*" for Managed Service for Apache Kafka.</rdfs:comment>
    <rdfs:domain rdf:resource="http://example.org/onto/class/google_managed_kafka_acl"/>
    <rdfs:range rdf:resource="http://www.w3.org/2001/XMLSchema#string"/>
  </owl:DatatypeProperty>
  <owl:DatatypeProperty rdf:about="http://example.org/onto/prop/google_managed_kafka_acl_operation">
    <rdfs:label>operation</rdfs:label>
    <rdfs:comment>The operation type. Allowed values are (case insensitive): ALL, READ,
WRITE, CREATE, DELETE, ALTER, DESCRIBE, CLUSTER_ACTION, DESCRIBE_CONFIGS,
ALTER_CONFIGS, and IDEMPOTENT_WRITE. See https://kafka.apache.org/documentation/#operations_resources_and_protocols
for valid combinations of resource_type and operation for different Kafka API requests.</rdfs:comment>
    <rdfs:domain rdf:resource="http://example.org/onto/class/google_managed_kafka_acl"/>
    <rdfs:range rdf:resource="http://www.w3.org/2001/XMLSchema#string"/>
  </owl:DatatypeProperty>
  <owl:DatatypeProperty rdf:about="http://example.org/onto/prop/google_managed_kafka_acl_permission_type">
    <rdfs:label>permission_type</rdfs:label>
    <rdfs:comment>The permission type. Accepted values are (case insensitive): ALLOW, DENY.</rdfs:comment>
    <rdfs:domain rdf:resource="http://example.org/onto/class/google_managed_kafka_acl"/>
    <rdfs:range rdf:resource="http://www.w3.org/2001/XMLSchema#string"/>
  </owl:DatatypeProperty>
  <owl:DatatypeProperty rdf:about="http://example.org/onto/prop/google_managed_kafka_acl_principal">
    <rdfs:label>principal</rdfs:label>
    <rdfs:comment>The principal. Specified as Google Cloud account, with the Kafka StandardAuthorizer prefix User:". For example: "User:test-kafka-client@test-project.iam.gserviceaccount.com". Can be the wildcard "User:*" to refer to all users.</rdfs:comment>
    <rdfs:domain rdf:resource="http://example.org/onto/class/google_managed_kafka_acl"/>
    <rdfs:range rdf:resource="http://www.w3.org/2001/XMLSchema#string"/>
  </owl:DatatypeProperty>
  <owl:DatatypeProperty rdf:about="http://example.org/onto/prop/google_managed_kafka_acl_create">
    <rdfs:label>create</rdfs:label>
    <rdfs:domain rdf:resource="http://example.org/onto/class/google_managed_kafka_acl"/>
    <rdfs:range rdf:resource="http://www.w3.org/2001/XMLSchema#string"/>
  </owl:DatatypeProperty>
  <owl:DatatypeProperty rdf:about="http://example.org/onto/prop/google_managed_kafka_acl_delete">
    <rdfs:label>delete</rdfs:label>
    <rdfs:domain rdf:resource="http://example.org/onto/class/google_managed_kafka_acl"/>
    <rdfs:range rdf:resource="http://www.w3.org/2001/XMLSchema#string"/>
  </owl:DatatypeProperty>
  <owl:DatatypeProperty rdf:about="http://example.org/onto/prop/google_managed_kafka_acl_update">
    <rdfs:label>update</rdfs:label>
    <rdfs:domain rdf:resource="http://example.org/onto/class/google_managed_kafka_acl"/>
    <rdfs:range rdf:resource="http://www.w3.org/2001/XMLSchema#string"/>
  </owl:DatatypeProperty>
</rdf:RDF>
