<?xml version="1.0" encoding="UTF-8"?>
<rdf:RDF
  xmlns:rdf="http://www.w3.org/1999/02/22-rdf-syntax-ns#"
  xmlns:rdfs="http://www.w3.org/2000/01/rdf-schema#"
  xmlns:owl="http://www.w3.org/2002/07/owl#"
  xmlns:xsd="http://www.w3.org/2001/XMLSchema#"
  xml:base="http://example.org/onto/">
  <owl:Class rdf:about="http://example.org/onto/class/google_notebooks_runtime">
    <rdfs:label>google_notebooks_runtime</rdfs:label>
    <rdfs:comment>#
#     ***     AUTO GENERATED CODE    ***    Type: MMv1     ***
#
# ----------------------------------------------------------------------------
#
#     This code is generated by Magic Modules using the following:
#
#     Configuration: https:#github.com/GoogleCloudPlatform/magic-modules/tree/main/mmv1/products/notebooks/Runtime.yaml
#     Template:      https:#github.com/GoogleCloudPlatform/magic-modules/tree/main/mmv1/templates/terraform/resource.html.markdown.tmpl
#
#     DO NOT EDIT this file directly. Any changes made to this file will be
#     overwritten during the next generation cycle.
#
# ----------------------------------------------------------------------------
subcategory: "Cloud AI Notebooks"
description: |-
  A Cloud AI Platform Notebook runtime.
---</rdfs:comment>
  </owl:Class>
  <owl:DatatypeProperty rdf:about="http://example.org/onto/prop/google_notebooks_runtime_effective_labels">
    <rdfs:label>effective_labels</rdfs:label>
    <rdfs:comment>All of labels (key/value pairs) present on the resource in GCP, including the labels configured through Terraform, other clients and services.</rdfs:comment>
    <rdfs:domain rdf:resource="http://example.org/onto/class/google_notebooks_runtime"/>
    <rdfs:range rdf:resource="http://www.w3.org/2001/XMLSchema#string"/>
  </owl:DatatypeProperty>
  <owl:DatatypeProperty rdf:about="http://example.org/onto/prop/google_notebooks_runtime_health_state">
    <rdfs:label>health_state</rdfs:label>
    <rdfs:comment>The health state of this runtime. For a list of possible output
values, see 'https://cloud.google.com/vertex-ai/docs/workbench/
reference/rest/v1/projects.locations.runtimes#healthstate'.</rdfs:comment>
    <rdfs:domain rdf:resource="http://example.org/onto/class/google_notebooks_runtime"/>
    <rdfs:range rdf:resource="http://www.w3.org/2001/XMLSchema#string"/>
  </owl:DatatypeProperty>
  <owl:DatatypeProperty rdf:about="http://example.org/onto/prop/google_notebooks_runtime_id">
    <rdfs:label>id</rdfs:label>
    <rdfs:domain rdf:resource="http://example.org/onto/class/google_notebooks_runtime"/>
    <rdfs:range rdf:resource="http://www.w3.org/2001/XMLSchema#string"/>
  </owl:DatatypeProperty>
  <owl:DatatypeProperty rdf:about="http://example.org/onto/prop/google_notebooks_runtime_labels">
    <rdfs:label>labels</rdfs:label>
    <rdfs:comment>The labels to associate with this runtime. Label **keys** must
contain 1 to 63 characters, and must conform to [RFC 1035]
(https://www.ietf.org/rfc/rfc1035.txt). Label **values** may be
empty, but, if present, must contain 1 to 63 characters, and must
conform to [RFC 1035](https://www.ietf.org/rfc/rfc1035.txt). No
more than 32 labels can be associated with a cluster.


**Note**: This field is non-authoritative, and will only manage the labels present in your configuration.
Please refer to the field 'effective_labels' for all of the labels present on the resource.</rdfs:comment>
    <rdfs:domain rdf:resource="http://example.org/onto/class/google_notebooks_runtime"/>
    <rdfs:range rdf:resource="http://www.w3.org/2001/XMLSchema#string"/>
  </owl:DatatypeProperty>
  <owl:DatatypeProperty rdf:about="http://example.org/onto/prop/google_notebooks_runtime_location">
    <rdfs:label>location</rdfs:label>
    <rdfs:comment>A reference to the zone where the machine resides.</rdfs:comment>
    <rdfs:domain rdf:resource="http://example.org/onto/class/google_notebooks_runtime"/>
    <rdfs:range rdf:resource="http://www.w3.org/2001/XMLSchema#string"/>
  </owl:DatatypeProperty>
  <owl:DatatypeProperty rdf:about="http://example.org/onto/prop/google_notebooks_runtime_metrics">
    <rdfs:label>metrics</rdfs:label>
    <rdfs:comment>Contains Runtime daemon metrics such as Service status and JupyterLab
status</rdfs:comment>
    <rdfs:domain rdf:resource="http://example.org/onto/class/google_notebooks_runtime"/>
    <rdfs:range rdf:resource="http://www.w3.org/2001/XMLSchema#string"/>
  </owl:DatatypeProperty>
  <owl:DatatypeProperty rdf:about="http://example.org/onto/prop/google_notebooks_runtime_name">
    <rdfs:label>name</rdfs:label>
    <rdfs:comment>The name specified for the Notebook runtime.</rdfs:comment>
    <rdfs:domain rdf:resource="http://example.org/onto/class/google_notebooks_runtime"/>
    <rdfs:range rdf:resource="http://www.w3.org/2001/XMLSchema#string"/>
  </owl:DatatypeProperty>
  <owl:DatatypeProperty rdf:about="http://example.org/onto/prop/google_notebooks_runtime_project">
    <rdfs:label>project</rdfs:label>
    <rdfs:domain rdf:resource="http://example.org/onto/class/google_notebooks_runtime"/>
    <rdfs:range rdf:resource="http://www.w3.org/2001/XMLSchema#string"/>
  </owl:DatatypeProperty>
  <owl:DatatypeProperty rdf:about="http://example.org/onto/prop/google_notebooks_runtime_state">
    <rdfs:label>state</rdfs:label>
    <rdfs:comment>The state of this runtime.</rdfs:comment>
    <rdfs:domain rdf:resource="http://example.org/onto/class/google_notebooks_runtime"/>
    <rdfs:range rdf:resource="http://www.w3.org/2001/XMLSchema#string"/>
  </owl:DatatypeProperty>
  <owl:DatatypeProperty rdf:about="http://example.org/onto/prop/google_notebooks_runtime_terraform_labels">
    <rdfs:label>terraform_labels</rdfs:label>
    <rdfs:comment>The combination of labels configured directly on the resource
 and default labels configured on the provider.</rdfs:comment>
    <rdfs:domain rdf:resource="http://example.org/onto/class/google_notebooks_runtime"/>
    <rdfs:range rdf:resource="http://www.w3.org/2001/XMLSchema#string"/>
  </owl:DatatypeProperty>
  <owl:DatatypeProperty rdf:about="http://example.org/onto/prop/google_notebooks_runtime_access_type">
    <rdfs:label>access_type</rdfs:label>
    <rdfs:comment>The type of access mode this instance. For valid values, see
'https://cloud.google.com/vertex-ai/docs/workbench/reference/
rest/v1/projects.locations.runtimes#RuntimeAccessType'.</rdfs:comment>
    <rdfs:domain rdf:resource="http://example.org/onto/class/google_notebooks_runtime"/>
    <rdfs:range rdf:resource="http://www.w3.org/2001/XMLSchema#string"/>
  </owl:DatatypeProperty>
  <owl:DatatypeProperty rdf:about="http://example.org/onto/prop/google_notebooks_runtime_proxy_uri">
    <rdfs:label>proxy_uri</rdfs:label>
    <rdfs:comment>The proxy endpoint that is used to access the runtime.</rdfs:comment>
    <rdfs:domain rdf:resource="http://example.org/onto/class/google_notebooks_runtime"/>
    <rdfs:range rdf:resource="http://www.w3.org/2001/XMLSchema#string"/>
  </owl:DatatypeProperty>
  <owl:DatatypeProperty rdf:about="http://example.org/onto/prop/google_notebooks_runtime_runtime_owner">
    <rdfs:label>runtime_owner</rdfs:label>
    <rdfs:comment>The owner of this runtime after creation. Format: 'alias@example.com'.
Currently supports one owner only.</rdfs:comment>
    <rdfs:domain rdf:resource="http://example.org/onto/class/google_notebooks_runtime"/>
    <rdfs:range rdf:resource="http://www.w3.org/2001/XMLSchema#string"/>
  </owl:DatatypeProperty>
  <owl:DatatypeProperty rdf:about="http://example.org/onto/prop/google_notebooks_runtime_custom_gpu_driver_path">
    <rdfs:label>custom_gpu_driver_path</rdfs:label>
    <rdfs:comment>Specify a custom Cloud Storage path where the GPU driver is stored.
If not specified, we'll automatically choose from official GPU drivers.</rdfs:comment>
    <rdfs:domain rdf:resource="http://example.org/onto/class/google_notebooks_runtime"/>
    <rdfs:range rdf:resource="http://www.w3.org/2001/XMLSchema#string"/>
  </owl:DatatypeProperty>
  <owl:DatatypeProperty rdf:about="http://example.org/onto/prop/google_notebooks_runtime_enable_health_monitoring">
    <rdfs:label>enable_health_monitoring</rdfs:label>
    <rdfs:comment>Verifies core internal services are running. Default: True.</rdfs:comment>
    <rdfs:domain rdf:resource="http://example.org/onto/class/google_notebooks_runtime"/>
    <rdfs:range rdf:resource="http://www.w3.org/2001/XMLSchema#string"/>
  </owl:DatatypeProperty>
  <owl:DatatypeProperty rdf:about="http://example.org/onto/prop/google_notebooks_runtime_idle_shutdown">
    <rdfs:label>idle_shutdown</rdfs:label>
    <rdfs:comment>Runtime will automatically shutdown after idle_shutdown_time.
Default: True</rdfs:comment>
    <rdfs:domain rdf:resource="http://example.org/onto/class/google_notebooks_runtime"/>
    <rdfs:range rdf:resource="http://www.w3.org/2001/XMLSchema#string"/>
  </owl:DatatypeProperty>
  <owl:DatatypeProperty rdf:about="http://example.org/onto/prop/google_notebooks_runtime_idle_shutdown_timeout">
    <rdfs:label>idle_shutdown_timeout</rdfs:label>
    <rdfs:comment>Time in minutes to wait before shuting down runtime.
Default: 180 minutes</rdfs:comment>
    <rdfs:domain rdf:resource="http://example.org/onto/class/google_notebooks_runtime"/>
    <rdfs:range rdf:resource="http://www.w3.org/2001/XMLSchema#string"/>
  </owl:DatatypeProperty>
  <owl:DatatypeProperty rdf:about="http://example.org/onto/prop/google_notebooks_runtime_install_gpu_driver">
    <rdfs:label>install_gpu_driver</rdfs:label>
    <rdfs:comment>Install Nvidia Driver automatically.</rdfs:comment>
    <rdfs:domain rdf:resource="http://example.org/onto/class/google_notebooks_runtime"/>
    <rdfs:range rdf:resource="http://www.w3.org/2001/XMLSchema#string"/>
  </owl:DatatypeProperty>
  <owl:DatatypeProperty rdf:about="http://example.org/onto/prop/google_notebooks_runtime_notebook_upgrade_schedule">
    <rdfs:label>notebook_upgrade_schedule</rdfs:label>
    <rdfs:comment>Cron expression in UTC timezone for schedule instance auto upgrade.
Please follow the [cron format](https://en.wikipedia.org/wiki/Cron).</rdfs:comment>
    <rdfs:domain rdf:resource="http://example.org/onto/class/google_notebooks_runtime"/>
    <rdfs:range rdf:resource="http://www.w3.org/2001/XMLSchema#string"/>
  </owl:DatatypeProperty>
  <owl:DatatypeProperty rdf:about="http://example.org/onto/prop/google_notebooks_runtime_post_startup_script">
    <rdfs:label>post_startup_script</rdfs:label>
    <rdfs:comment>Path to a Bash script that automatically runs after a notebook instance
fully boots up. The path must be a URL or
Cloud Storage path (gs://path-to-file/file-name).</rdfs:comment>
    <rdfs:domain rdf:resource="http://example.org/onto/class/google_notebooks_runtime"/>
    <rdfs:range rdf:resource="http://www.w3.org/2001/XMLSchema#string"/>
  </owl:DatatypeProperty>
  <owl:DatatypeProperty rdf:about="http://example.org/onto/prop/google_notebooks_runtime_post_startup_script_behavior">
    <rdfs:label>post_startup_script_behavior</rdfs:label>
    <rdfs:comment>Behavior for the post startup script. Possible values: ["POST_STARTUP_SCRIPT_BEHAVIOR_UNSPECIFIED", "RUN_EVERY_START", "DOWNLOAD_AND_RUN_EVERY_START"]</rdfs:comment>
    <rdfs:domain rdf:resource="http://example.org/onto/class/google_notebooks_runtime"/>
    <rdfs:range rdf:resource="http://www.w3.org/2001/XMLSchema#string"/>
  </owl:DatatypeProperty>
  <owl:DatatypeProperty rdf:about="http://example.org/onto/prop/google_notebooks_runtime_upgradeable">
    <rdfs:label>upgradeable</rdfs:label>
    <rdfs:comment>Bool indicating whether an newer image is available in an image family.</rdfs:comment>
    <rdfs:domain rdf:resource="http://example.org/onto/class/google_notebooks_runtime"/>
    <rdfs:range rdf:resource="http://www.w3.org/2001/XMLSchema#string"/>
  </owl:DatatypeProperty>
  <owl:DatatypeProperty rdf:about="http://example.org/onto/prop/google_notebooks_runtime_repository">
    <rdfs:label>repository</rdfs:label>
    <rdfs:comment>The path to the container image repository.
For example: gcr.io/{project_id}/{imageName}</rdfs:comment>
    <rdfs:domain rdf:resource="http://example.org/onto/class/google_notebooks_runtime"/>
    <rdfs:range rdf:resource="http://www.w3.org/2001/XMLSchema#string"/>
  </owl:DatatypeProperty>
  <owl:DatatypeProperty rdf:about="http://example.org/onto/prop/google_notebooks_runtime_tag">
    <rdfs:label>tag</rdfs:label>
    <rdfs:comment>The tag of the container image. If not specified, this defaults to the latest tag.</rdfs:comment>
    <rdfs:domain rdf:resource="http://example.org/onto/class/google_notebooks_runtime"/>
    <rdfs:range rdf:resource="http://www.w3.org/2001/XMLSchema#string"/>
  </owl:DatatypeProperty>
  <owl:DatatypeProperty rdf:about="http://example.org/onto/prop/google_notebooks_runtime_create">
    <rdfs:label>create</rdfs:label>
    <rdfs:domain rdf:resource="http://example.org/onto/class/google_notebooks_runtime"/>
    <rdfs:range rdf:resource="http://www.w3.org/2001/XMLSchema#string"/>
  </owl:DatatypeProperty>
  <owl:DatatypeProperty rdf:about="http://example.org/onto/prop/google_notebooks_runtime_delete">
    <rdfs:label>delete</rdfs:label>
    <rdfs:domain rdf:resource="http://example.org/onto/class/google_notebooks_runtime"/>
    <rdfs:range rdf:resource="http://www.w3.org/2001/XMLSchema#string"/>
  </owl:DatatypeProperty>
  <owl:DatatypeProperty rdf:about="http://example.org/onto/prop/google_notebooks_runtime_update">
    <rdfs:label>update</rdfs:label>
    <rdfs:domain rdf:resource="http://example.org/onto/class/google_notebooks_runtime"/>
    <rdfs:range rdf:resource="http://www.w3.org/2001/XMLSchema#string"/>
  </owl:DatatypeProperty>
  <owl:DatatypeProperty rdf:about="http://example.org/onto/prop/google_notebooks_runtime_instance_id">
    <rdfs:label>instance_id</rdfs:label>
    <rdfs:comment>The unique identifier of the Managed Compute Engine instance.</rdfs:comment>
    <rdfs:domain rdf:resource="http://example.org/onto/class/google_notebooks_runtime"/>
    <rdfs:range rdf:resource="http://www.w3.org/2001/XMLSchema#string"/>
  </owl:DatatypeProperty>
  <owl:DatatypeProperty rdf:about="http://example.org/onto/prop/google_notebooks_runtime_instance_name">
    <rdfs:label>instance_name</rdfs:label>
    <rdfs:comment>The user-friendly name of the Managed Compute Engine instance.</rdfs:comment>
    <rdfs:domain rdf:resource="http://example.org/onto/class/google_notebooks_runtime"/>
    <rdfs:range rdf:resource="http://www.w3.org/2001/XMLSchema#string"/>
  </owl:DatatypeProperty>
  <owl:DatatypeProperty rdf:about="http://example.org/onto/prop/google_notebooks_runtime_guest_attributes">
    <rdfs:label>guest_attributes</rdfs:label>
    <rdfs:comment>The Compute Engine guest attributes. (see [Project and instance
guest attributes](https://cloud.google.com/compute/docs/
storing-retrieving-metadata#guest_attributes)).</rdfs:comment>
    <rdfs:domain rdf:resource="http://example.org/onto/class/google_notebooks_runtime"/>
    <rdfs:range rdf:resource="http://www.w3.org/2001/XMLSchema#string"/>
  </owl:DatatypeProperty>
  <owl:DatatypeProperty rdf:about="http://example.org/onto/prop/google_notebooks_runtime_internal_ip_only">
    <rdfs:label>internal_ip_only</rdfs:label>
    <rdfs:comment>If true, runtime will only have internal IP addresses. By default,
runtimes are not restricted to internal IP addresses, and will
have ephemeral external IP addresses assigned to each vm. This
'internal_ip_only' restriction can only be enabled for subnetwork
enabled networks, and all dependencies must be configured to be
accessible without external IP addresses.</rdfs:comment>
    <rdfs:domain rdf:resource="http://example.org/onto/class/google_notebooks_runtime"/>
    <rdfs:range rdf:resource="http://www.w3.org/2001/XMLSchema#string"/>
  </owl:DatatypeProperty>
  <owl:DatatypeProperty rdf:about="http://example.org/onto/prop/google_notebooks_runtime_labels">
    <rdfs:label>labels</rdfs:label>
    <rdfs:comment>The labels to associate with this runtime. Label **keys** must
contain 1 to 63 characters, and must conform to [RFC 1035]
(https://www.ietf.org/rfc/rfc1035.txt). Label **values** may be
empty, but, if present, must contain 1 to 63 characters, and must
conform to [RFC 1035](https://www.ietf.org/rfc/rfc1035.txt). No
more than 32 labels can be associated with a cluster.</rdfs:comment>
    <rdfs:domain rdf:resource="http://example.org/onto/class/google_notebooks_runtime"/>
    <rdfs:range rdf:resource="http://www.w3.org/2001/XMLSchema#string"/>
  </owl:DatatypeProperty>
  <owl:DatatypeProperty rdf:about="http://example.org/onto/prop/google_notebooks_runtime_machine_type">
    <rdfs:label>machine_type</rdfs:label>
    <rdfs:comment>The Compute Engine machine type used for runtimes.</rdfs:comment>
    <rdfs:domain rdf:resource="http://example.org/onto/class/google_notebooks_runtime"/>
    <rdfs:range rdf:resource="http://www.w3.org/2001/XMLSchema#string"/>
  </owl:DatatypeProperty>
  <owl:DatatypeProperty rdf:about="http://example.org/onto/prop/google_notebooks_runtime_metadata">
    <rdfs:label>metadata</rdfs:label>
    <rdfs:comment>The Compute Engine metadata entries to add to virtual machine.
(see [Project and instance metadata](https://cloud.google.com
/compute/docs/storing-retrieving-metadata#project_and_instance
_metadata)).</rdfs:comment>
    <rdfs:domain rdf:resource="http://example.org/onto/class/google_notebooks_runtime"/>
    <rdfs:range rdf:resource="http://www.w3.org/2001/XMLSchema#string"/>
  </owl:DatatypeProperty>
  <owl:DatatypeProperty rdf:about="http://example.org/onto/prop/google_notebooks_runtime_network">
    <rdfs:label>network</rdfs:label>
    <rdfs:comment>The Compute Engine network to be used for machine communications.
Cannot be specified with subnetwork. If neither 'network' nor
'subnet' is specified, the "default" network of the project is
used, if it exists. A full URL or partial URI. Examples:
  * 'https://www.googleapis.com/compute/v1/projects/[project_id]/
  regions/global/default'
  * 'projects/[project_id]/regions/global/default'
Runtimes are managed resources inside Google Infrastructure.
Runtimes support the following network configurations:
  * Google Managed Network (Network & subnet are empty)
  * Consumer Project VPC (network & subnet are required). Requires
  configuring Private Service Access.
  * Shared VPC (network & subnet are required). Requires
  configuring Private Service Access.</rdfs:comment>
    <rdfs:domain rdf:resource="http://example.org/onto/class/google_notebooks_runtime"/>
    <rdfs:range rdf:resource="http://www.w3.org/2001/XMLSchema#string"/>
  </owl:DatatypeProperty>
  <owl:DatatypeProperty rdf:about="http://example.org/onto/prop/google_notebooks_runtime_nic_type">
    <rdfs:label>nic_type</rdfs:label>
    <rdfs:comment>The type of vNIC to be used on this interface. This may be gVNIC
or VirtioNet. Possible values: ["UNSPECIFIED_NIC_TYPE", "VIRTIO_NET", "GVNIC"]</rdfs:comment>
    <rdfs:domain rdf:resource="http://example.org/onto/class/google_notebooks_runtime"/>
    <rdfs:range rdf:resource="http://www.w3.org/2001/XMLSchema#string"/>
  </owl:DatatypeProperty>
  <owl:DatatypeProperty rdf:about="http://example.org/onto/prop/google_notebooks_runtime_reserved_ip_range">
    <rdfs:label>reserved_ip_range</rdfs:label>
    <rdfs:comment>Reserved IP Range name is used for VPC Peering. The
subnetwork allocation will use the range *name* if it's assigned.</rdfs:comment>
    <rdfs:domain rdf:resource="http://example.org/onto/class/google_notebooks_runtime"/>
    <rdfs:range rdf:resource="http://www.w3.org/2001/XMLSchema#string"/>
  </owl:DatatypeProperty>
  <owl:DatatypeProperty rdf:about="http://example.org/onto/prop/google_notebooks_runtime_subnet">
    <rdfs:label>subnet</rdfs:label>
    <rdfs:comment>The Compute Engine subnetwork to be used for machine
communications. Cannot be specified with network. A full URL or
partial URI are valid. Examples:
  * 'https://www.googleapis.com/compute/v1/projects/[project_id]/
  regions/us-east1/subnetworks/sub0'
  * 'projects/[project_id]/regions/us-east1/subnetworks/sub0'</rdfs:comment>
    <rdfs:domain rdf:resource="http://example.org/onto/class/google_notebooks_runtime"/>
    <rdfs:range rdf:resource="http://www.w3.org/2001/XMLSchema#string"/>
  </owl:DatatypeProperty>
  <owl:DatatypeProperty rdf:about="http://example.org/onto/prop/google_notebooks_runtime_tags">
    <rdfs:label>tags</rdfs:label>
    <rdfs:comment>The Compute Engine tags to add to runtime (see [Tagging instances]
(https://cloud.google.com/compute/docs/
label-or-tag-resources#tags)).</rdfs:comment>
    <rdfs:domain rdf:resource="http://example.org/onto/class/google_notebooks_runtime"/>
    <rdfs:range rdf:resource="http://www.w3.org/2001/XMLSchema#string"/>
  </owl:DatatypeProperty>
  <owl:DatatypeProperty rdf:about="http://example.org/onto/prop/google_notebooks_runtime_zone">
    <rdfs:label>zone</rdfs:label>
    <rdfs:comment>The zone where the virtual machine is located.</rdfs:comment>
    <rdfs:domain rdf:resource="http://example.org/onto/class/google_notebooks_runtime"/>
    <rdfs:range rdf:resource="http://www.w3.org/2001/XMLSchema#string"/>
  </owl:DatatypeProperty>
  <owl:DatatypeProperty rdf:about="http://example.org/onto/prop/google_notebooks_runtime_core_count">
    <rdfs:label>core_count</rdfs:label>
    <rdfs:comment>Count of cores of this accelerator.</rdfs:comment>
    <rdfs:domain rdf:resource="http://example.org/onto/class/google_notebooks_runtime"/>
    <rdfs:range rdf:resource="http://www.w3.org/2001/XMLSchema#string"/>
  </owl:DatatypeProperty>
  <owl:DatatypeProperty rdf:about="http://example.org/onto/prop/google_notebooks_runtime_type">
    <rdfs:label>type</rdfs:label>
    <rdfs:comment>Accelerator model. For valid values, see
'https://cloud.google.com/vertex-ai/docs/workbench/reference/
rest/v1/projects.locations.runtimes#AcceleratorType'</rdfs:comment>
    <rdfs:domain rdf:resource="http://example.org/onto/class/google_notebooks_runtime"/>
    <rdfs:range rdf:resource="http://www.w3.org/2001/XMLSchema#string"/>
  </owl:DatatypeProperty>
  <owl:DatatypeProperty rdf:about="http://example.org/onto/prop/google_notebooks_runtime_repository">
    <rdfs:label>repository</rdfs:label>
    <rdfs:comment>The path to the container image repository.
For example: gcr.io/{project_id}/{imageName}</rdfs:comment>
    <rdfs:domain rdf:resource="http://example.org/onto/class/google_notebooks_runtime"/>
    <rdfs:range rdf:resource="http://www.w3.org/2001/XMLSchema#string"/>
  </owl:DatatypeProperty>
  <owl:DatatypeProperty rdf:about="http://example.org/onto/prop/google_notebooks_runtime_tag">
    <rdfs:label>tag</rdfs:label>
    <rdfs:comment>The tag of the container image. If not specified, this defaults to the latest tag.</rdfs:comment>
    <rdfs:domain rdf:resource="http://example.org/onto/class/google_notebooks_runtime"/>
    <rdfs:range rdf:resource="http://www.w3.org/2001/XMLSchema#string"/>
  </owl:DatatypeProperty>
  <owl:DatatypeProperty rdf:about="http://example.org/onto/prop/google_notebooks_runtime_auto_delete">
    <rdfs:label>auto_delete</rdfs:label>
    <rdfs:comment>Optional. Specifies whether the disk will be auto-deleted
when the instance is deleted (but not when the disk is
detached from the instance).</rdfs:comment>
    <rdfs:domain rdf:resource="http://example.org/onto/class/google_notebooks_runtime"/>
    <rdfs:range rdf:resource="http://www.w3.org/2001/XMLSchema#string"/>
  </owl:DatatypeProperty>
  <owl:DatatypeProperty rdf:about="http://example.org/onto/prop/google_notebooks_runtime_boot">
    <rdfs:label>boot</rdfs:label>
    <rdfs:comment>Optional. Indicates that this is a boot disk. The virtual
machine will use the first partition of the disk for its
root filesystem.</rdfs:comment>
    <rdfs:domain rdf:resource="http://example.org/onto/class/google_notebooks_runtime"/>
    <rdfs:range rdf:resource="http://www.w3.org/2001/XMLSchema#string"/>
  </owl:DatatypeProperty>
  <owl:DatatypeProperty rdf:about="http://example.org/onto/prop/google_notebooks_runtime_device_name">
    <rdfs:label>device_name</rdfs:label>
    <rdfs:comment>Optional. Specifies a unique device name of your choice
that is reflected into the /dev/disk/by-id/google-* tree
of a Linux operating system running within the instance.
This name can be used to reference the device for mounting,
resizing, and so on, from within the instance.
If not specified, the server chooses a default device name
to apply to this disk, in the form persistent-disk-x, where
x is a number assigned by Google Compute Engine. This field
is only applicable for persistent disks.</rdfs:comment>
    <rdfs:domain rdf:resource="http://example.org/onto/class/google_notebooks_runtime"/>
    <rdfs:range rdf:resource="http://www.w3.org/2001/XMLSchema#string"/>
  </owl:DatatypeProperty>
  <owl:DatatypeProperty rdf:about="http://example.org/onto/prop/google_notebooks_runtime_guest_os_features">
    <rdfs:label>guest_os_features</rdfs:label>
    <rdfs:comment>Indicates a list of features to enable on the guest operating
system. Applicable only for bootable images. To see a list of
available features, read 'https://cloud.google.com/compute/docs/
images/create-delete-deprecate-private-images#guest-os-features'
options. ''</rdfs:comment>
    <rdfs:domain rdf:resource="http://example.org/onto/class/google_notebooks_runtime"/>
    <rdfs:range rdf:resource="http://www.w3.org/2001/XMLSchema#string"/>
  </owl:DatatypeProperty>
  <owl:DatatypeProperty rdf:about="http://example.org/onto/prop/google_notebooks_runtime_index">
    <rdfs:label>index</rdfs:label>
    <rdfs:comment>Output only. A zero-based index to this disk, where 0 is
reserved for the boot disk. If you have many disks attached
to an instance, each disk would have a unique index number.</rdfs:comment>
    <rdfs:domain rdf:resource="http://example.org/onto/class/google_notebooks_runtime"/>
    <rdfs:range rdf:resource="http://www.w3.org/2001/XMLSchema#string"/>
  </owl:DatatypeProperty>
  <owl:DatatypeProperty rdf:about="http://example.org/onto/prop/google_notebooks_runtime_interface">
    <rdfs:label>interface</rdfs:label>
    <rdfs:comment>"Specifies the disk interface to use for attaching this disk,
which is either SCSI or NVME. The default is SCSI. Persistent
disks must always use SCSI and the request will fail if you attempt
to attach a persistent disk in any other format than SCSI. Local SSDs
can use either NVME or SCSI. For performance characteristics of SCSI
over NVMe, see Local SSD performance. Valid values: * NVME * SCSI".</rdfs:comment>
    <rdfs:domain rdf:resource="http://example.org/onto/class/google_notebooks_runtime"/>
    <rdfs:range rdf:resource="http://www.w3.org/2001/XMLSchema#string"/>
  </owl:DatatypeProperty>
  <owl:DatatypeProperty rdf:about="http://example.org/onto/prop/google_notebooks_runtime_kind">
    <rdfs:label>kind</rdfs:label>
    <rdfs:comment>Type of the resource. Always compute#attachedDisk for attached
disks.</rdfs:comment>
    <rdfs:domain rdf:resource="http://example.org/onto/class/google_notebooks_runtime"/>
    <rdfs:range rdf:resource="http://www.w3.org/2001/XMLSchema#string"/>
  </owl:DatatypeProperty>
  <owl:DatatypeProperty rdf:about="http://example.org/onto/prop/google_notebooks_runtime_licenses">
    <rdfs:label>licenses</rdfs:label>
    <rdfs:comment>Output only. Any valid publicly visible licenses.</rdfs:comment>
    <rdfs:domain rdf:resource="http://example.org/onto/class/google_notebooks_runtime"/>
    <rdfs:range rdf:resource="http://www.w3.org/2001/XMLSchema#string"/>
  </owl:DatatypeProperty>
  <owl:DatatypeProperty rdf:about="http://example.org/onto/prop/google_notebooks_runtime_mode">
    <rdfs:label>mode</rdfs:label>
    <rdfs:comment>The mode in which to attach this disk, either READ_WRITE
or READ_ONLY. If not specified, the default is to attach
the disk in READ_WRITE mode.</rdfs:comment>
    <rdfs:domain rdf:resource="http://example.org/onto/class/google_notebooks_runtime"/>
    <rdfs:range rdf:resource="http://www.w3.org/2001/XMLSchema#string"/>
  </owl:DatatypeProperty>
  <owl:DatatypeProperty rdf:about="http://example.org/onto/prop/google_notebooks_runtime_source">
    <rdfs:label>source</rdfs:label>
    <rdfs:comment>Specifies a valid partial or full URL to an existing
Persistent Disk resource.</rdfs:comment>
    <rdfs:domain rdf:resource="http://example.org/onto/class/google_notebooks_runtime"/>
    <rdfs:range rdf:resource="http://www.w3.org/2001/XMLSchema#string"/>
  </owl:DatatypeProperty>
  <owl:DatatypeProperty rdf:about="http://example.org/onto/prop/google_notebooks_runtime_type">
    <rdfs:label>type</rdfs:label>
    <rdfs:comment>Specifies the type of the disk, either SCRATCH or PERSISTENT.
If not specified, the default is PERSISTENT.</rdfs:comment>
    <rdfs:domain rdf:resource="http://example.org/onto/class/google_notebooks_runtime"/>
    <rdfs:range rdf:resource="http://www.w3.org/2001/XMLSchema#string"/>
  </owl:DatatypeProperty>
  <owl:DatatypeProperty rdf:about="http://example.org/onto/prop/google_notebooks_runtime_description">
    <rdfs:label>description</rdfs:label>
    <rdfs:comment>Provide this property when creating the disk.</rdfs:comment>
    <rdfs:domain rdf:resource="http://example.org/onto/class/google_notebooks_runtime"/>
    <rdfs:range rdf:resource="http://www.w3.org/2001/XMLSchema#string"/>
  </owl:DatatypeProperty>
  <owl:DatatypeProperty rdf:about="http://example.org/onto/prop/google_notebooks_runtime_disk_name">
    <rdfs:label>disk_name</rdfs:label>
    <rdfs:comment>Specifies the disk name. If not specified, the default is
to use the name of the instance. If the disk with the
instance name exists already in the given zone/region, a
new name will be automatically generated.</rdfs:comment>
    <rdfs:domain rdf:resource="http://example.org/onto/class/google_notebooks_runtime"/>
    <rdfs:range rdf:resource="http://www.w3.org/2001/XMLSchema#string"/>
  </owl:DatatypeProperty>
  <owl:DatatypeProperty rdf:about="http://example.org/onto/prop/google_notebooks_runtime_disk_size_gb">
    <rdfs:label>disk_size_gb</rdfs:label>
    <rdfs:comment>Specifies the size of the disk in base-2 GB. If not
specified, the disk will be the same size as the image
(usually 10GB). If specified, the size must be equal to
or larger than 10GB. Default 100 GB.</rdfs:comment>
    <rdfs:domain rdf:resource="http://example.org/onto/class/google_notebooks_runtime"/>
    <rdfs:range rdf:resource="http://www.w3.org/2001/XMLSchema#string"/>
  </owl:DatatypeProperty>
  <owl:DatatypeProperty rdf:about="http://example.org/onto/prop/google_notebooks_runtime_disk_type">
    <rdfs:label>disk_type</rdfs:label>
    <rdfs:comment>The type of the boot disk attached to this runtime,
defaults to standard persistent disk. For valid values,
see 'https://cloud.google.com/vertex-ai/docs/workbench/
reference/rest/v1/projects.locations.runtimes#disktype'</rdfs:comment>
    <rdfs:domain rdf:resource="http://example.org/onto/class/google_notebooks_runtime"/>
    <rdfs:range rdf:resource="http://www.w3.org/2001/XMLSchema#string"/>
  </owl:DatatypeProperty>
  <owl:DatatypeProperty rdf:about="http://example.org/onto/prop/google_notebooks_runtime_labels">
    <rdfs:label>labels</rdfs:label>
    <rdfs:comment>Labels to apply to this disk. These can be later modified
by the disks.setLabels method. This field is only
applicable for persistent disks.</rdfs:comment>
    <rdfs:domain rdf:resource="http://example.org/onto/class/google_notebooks_runtime"/>
    <rdfs:range rdf:resource="http://www.w3.org/2001/XMLSchema#string"/>
  </owl:DatatypeProperty>
  <owl:DatatypeProperty rdf:about="http://example.org/onto/prop/google_notebooks_runtime_kms_key">
    <rdfs:label>kms_key</rdfs:label>
    <rdfs:comment>The Cloud KMS resource identifier of the customer-managed
encryption key used to protect a resource, such as a disks.
It has the following format:
'projects/{PROJECT_ID}/locations/{REGION}/keyRings/
{KEY_RING_NAME}/cryptoKeys/{KEY_NAME}'</rdfs:comment>
    <rdfs:domain rdf:resource="http://example.org/onto/class/google_notebooks_runtime"/>
    <rdfs:range rdf:resource="http://www.w3.org/2001/XMLSchema#string"/>
  </owl:DatatypeProperty>
  <owl:DatatypeProperty rdf:about="http://example.org/onto/prop/google_notebooks_runtime_enable_integrity_monitoring">
    <rdfs:label>enable_integrity_monitoring</rdfs:label>
    <rdfs:comment>Defines whether the instance has integrity monitoring enabled.
Enables monitoring and attestation of the boot integrity of
the instance. The attestation is performed against the
integrity policy baseline. This baseline is initially derived
from the implicitly trusted boot image when the instance is
created. Enabled by default.</rdfs:comment>
    <rdfs:domain rdf:resource="http://example.org/onto/class/google_notebooks_runtime"/>
    <rdfs:range rdf:resource="http://www.w3.org/2001/XMLSchema#string"/>
  </owl:DatatypeProperty>
  <owl:DatatypeProperty rdf:about="http://example.org/onto/prop/google_notebooks_runtime_enable_secure_boot">
    <rdfs:label>enable_secure_boot</rdfs:label>
    <rdfs:comment>Defines whether the instance has Secure Boot enabled.Secure
Boot helps ensure that the system only runs authentic software
by verifying the digital signature of all boot components, and
halting the boot process if signature verification fails.
Disabled by default.</rdfs:comment>
    <rdfs:domain rdf:resource="http://example.org/onto/class/google_notebooks_runtime"/>
    <rdfs:range rdf:resource="http://www.w3.org/2001/XMLSchema#string"/>
  </owl:DatatypeProperty>
  <owl:DatatypeProperty rdf:about="http://example.org/onto/prop/google_notebooks_runtime_enable_vtpm">
    <rdfs:label>enable_vtpm</rdfs:label>
    <rdfs:comment>Defines whether the instance has the vTPM enabled. Enabled by
default.</rdfs:comment>
    <rdfs:domain rdf:resource="http://example.org/onto/class/google_notebooks_runtime"/>
    <rdfs:range rdf:resource="http://www.w3.org/2001/XMLSchema#string"/>
  </owl:DatatypeProperty>
</rdf:RDF>
