<?xml version="1.0" encoding="UTF-8"?>
<rdf:RDF
  xmlns:rdf="http://www.w3.org/1999/02/22-rdf-syntax-ns#"
  xmlns:rdfs="http://www.w3.org/2000/01/rdf-schema#"
  xmlns:owl="http://www.w3.org/2002/07/owl#"
  xmlns:xsd="http://www.w3.org/2001/XMLSchema#"
  xml:base="http://example.org/onto/">
  <owl:Class rdf:about="http://example.org/onto/class/google_network_services_authz_extension">
    <rdfs:label>google_network_services_authz_extension</rdfs:label>
    <rdfs:comment>#
#     ***     AUTO GENERATED CODE    ***    Type: MMv1     ***
#
# ----------------------------------------------------------------------------
#
#     This code is generated by Magic Modules using the following:
#
#     Configuration: https:#github.com/GoogleCloudPlatform/magic-modules/tree/main/mmv1/products/networkservices/AuthzExtension.yaml
#     Template:      https:#github.com/GoogleCloudPlatform/magic-modules/tree/main/mmv1/templates/terraform/resource.html.markdown.tmpl
#
#     DO NOT EDIT this file directly. Any changes made to this file will be
#     overwritten during the next generation cycle.
#
# ----------------------------------------------------------------------------
subcategory: "Network Services"
description: |-
  AuthzExtension is a resource that allows traffic forwarding to a callout backend service to make an authorization decision.
---</rdfs:comment>
  </owl:Class>
  <owl:DatatypeProperty rdf:about="http://example.org/onto/prop/google_network_services_authz_extension_authority">
    <rdfs:label>authority</rdfs:label>
    <rdfs:comment>The :authority header in the gRPC request sent from Envoy to the extension service.</rdfs:comment>
    <rdfs:domain rdf:resource="http://example.org/onto/class/google_network_services_authz_extension"/>
    <rdfs:range rdf:resource="http://www.w3.org/2001/XMLSchema#string"/>
  </owl:DatatypeProperty>
  <owl:DatatypeProperty rdf:about="http://example.org/onto/prop/google_network_services_authz_extension_create_time">
    <rdfs:label>create_time</rdfs:label>
    <rdfs:comment>The timestamp when the resource was created.</rdfs:comment>
    <rdfs:domain rdf:resource="http://example.org/onto/class/google_network_services_authz_extension"/>
    <rdfs:range rdf:resource="http://www.w3.org/2001/XMLSchema#string"/>
  </owl:DatatypeProperty>
  <owl:DatatypeProperty rdf:about="http://example.org/onto/prop/google_network_services_authz_extension_description">
    <rdfs:label>description</rdfs:label>
    <rdfs:comment>A human-readable description of the resource.</rdfs:comment>
    <rdfs:domain rdf:resource="http://example.org/onto/class/google_network_services_authz_extension"/>
    <rdfs:range rdf:resource="http://www.w3.org/2001/XMLSchema#string"/>
  </owl:DatatypeProperty>
  <owl:DatatypeProperty rdf:about="http://example.org/onto/prop/google_network_services_authz_extension_effective_labels">
    <rdfs:label>effective_labels</rdfs:label>
    <rdfs:comment>All of labels (key/value pairs) present on the resource in GCP, including the labels configured through Terraform, other clients and services.</rdfs:comment>
    <rdfs:domain rdf:resource="http://example.org/onto/class/google_network_services_authz_extension"/>
    <rdfs:range rdf:resource="http://www.w3.org/2001/XMLSchema#string"/>
  </owl:DatatypeProperty>
  <owl:DatatypeProperty rdf:about="http://example.org/onto/prop/google_network_services_authz_extension_fail_open">
    <rdfs:label>fail_open</rdfs:label>
    <rdfs:comment>Determines how the proxy behaves if the call to the extension fails or times out.
When set to TRUE, request or response processing continues without error. Any subsequent extensions in the extension chain are also executed. When set to FALSE or the default setting of FALSE is used, one of the following happens:
* If response headers have not been delivered to the downstream client, a generic 500 error is returned to the client. The error response can be tailored by configuring a custom error response in the load balancer.
* If response headers have been delivered, then the HTTP stream to the downstream client is reset.</rdfs:comment>
    <rdfs:domain rdf:resource="http://example.org/onto/class/google_network_services_authz_extension"/>
    <rdfs:range rdf:resource="http://www.w3.org/2001/XMLSchema#string"/>
  </owl:DatatypeProperty>
  <owl:DatatypeProperty rdf:about="http://example.org/onto/prop/google_network_services_authz_extension_forward_headers">
    <rdfs:label>forward_headers</rdfs:label>
    <rdfs:comment>List of the HTTP headers to forward to the extension (from the client). If omitted, all headers are sent. Each element is a string indicating the header name.</rdfs:comment>
    <rdfs:domain rdf:resource="http://example.org/onto/class/google_network_services_authz_extension"/>
    <rdfs:range rdf:resource="http://www.w3.org/2001/XMLSchema#string"/>
  </owl:DatatypeProperty>
  <owl:DatatypeProperty rdf:about="http://example.org/onto/prop/google_network_services_authz_extension_id">
    <rdfs:label>id</rdfs:label>
    <rdfs:domain rdf:resource="http://example.org/onto/class/google_network_services_authz_extension"/>
    <rdfs:range rdf:resource="http://www.w3.org/2001/XMLSchema#string"/>
  </owl:DatatypeProperty>
  <owl:DatatypeProperty rdf:about="http://example.org/onto/prop/google_network_services_authz_extension_labels">
    <rdfs:label>labels</rdfs:label>
    <rdfs:comment>Set of labels associated with the AuthzExtension resource.


**Note**: This field is non-authoritative, and will only manage the labels present in your configuration.
Please refer to the field 'effective_labels' for all of the labels present on the resource.</rdfs:comment>
    <rdfs:domain rdf:resource="http://example.org/onto/class/google_network_services_authz_extension"/>
    <rdfs:range rdf:resource="http://www.w3.org/2001/XMLSchema#string"/>
  </owl:DatatypeProperty>
  <owl:DatatypeProperty rdf:about="http://example.org/onto/prop/google_network_services_authz_extension_load_balancing_scheme">
    <rdfs:label>load_balancing_scheme</rdfs:label>
    <rdfs:comment>All backend services and forwarding rules referenced by this extension must share the same load balancing scheme.
For more information, refer to [Backend services overview](https://cloud.google.com/load-balancing/docs/backend-service). Possible values: ["INTERNAL_MANAGED", "EXTERNAL_MANAGED"]</rdfs:comment>
    <rdfs:domain rdf:resource="http://example.org/onto/class/google_network_services_authz_extension"/>
    <rdfs:range rdf:resource="http://www.w3.org/2001/XMLSchema#string"/>
  </owl:DatatypeProperty>
  <owl:DatatypeProperty rdf:about="http://example.org/onto/prop/google_network_services_authz_extension_location">
    <rdfs:label>location</rdfs:label>
    <rdfs:comment>The location of the resource.</rdfs:comment>
    <rdfs:domain rdf:resource="http://example.org/onto/class/google_network_services_authz_extension"/>
    <rdfs:range rdf:resource="http://www.w3.org/2001/XMLSchema#string"/>
  </owl:DatatypeProperty>
  <owl:DatatypeProperty rdf:about="http://example.org/onto/prop/google_network_services_authz_extension_metadata">
    <rdfs:label>metadata</rdfs:label>
    <rdfs:comment>The metadata provided here is included as part of the metadata_context (of type google.protobuf.Struct) in the ProcessingRequest message sent to the extension server. The metadata is available under the namespace com.google.authz_extension.<resourceName>. The following variables are supported in the metadata Struct:

{forwarding_rule_id} - substituted with the forwarding rule's fully qualified resource name.</rdfs:comment>
    <rdfs:domain rdf:resource="http://example.org/onto/class/google_network_services_authz_extension"/>
    <rdfs:range rdf:resource="http://www.w3.org/2001/XMLSchema#string"/>
  </owl:DatatypeProperty>
  <owl:DatatypeProperty rdf:about="http://example.org/onto/prop/google_network_services_authz_extension_name">
    <rdfs:label>name</rdfs:label>
    <rdfs:comment>Identifier. Name of the AuthzExtension resource.</rdfs:comment>
    <rdfs:domain rdf:resource="http://example.org/onto/class/google_network_services_authz_extension"/>
    <rdfs:range rdf:resource="http://www.w3.org/2001/XMLSchema#string"/>
  </owl:DatatypeProperty>
  <owl:DatatypeProperty rdf:about="http://example.org/onto/prop/google_network_services_authz_extension_project">
    <rdfs:label>project</rdfs:label>
    <rdfs:domain rdf:resource="http://example.org/onto/class/google_network_services_authz_extension"/>
    <rdfs:range rdf:resource="http://www.w3.org/2001/XMLSchema#string"/>
  </owl:DatatypeProperty>
  <owl:DatatypeProperty rdf:about="http://example.org/onto/prop/google_network_services_authz_extension_service">
    <rdfs:label>service</rdfs:label>
    <rdfs:comment>The reference to the service that runs the extension.
To configure a callout extension, service must be a fully-qualified reference to a [backend service](https://cloud.google.com/compute/docs/reference/rest/v1/backendServices) in the format:
https://www.googleapis.com/compute/v1/projects/{project}/regions/{region}/backendServices/{backendService} or https://www.googleapis.com/compute/v1/projects/{project}/global/backendServices/{backendService}.</rdfs:comment>
    <rdfs:domain rdf:resource="http://example.org/onto/class/google_network_services_authz_extension"/>
    <rdfs:range rdf:resource="http://www.w3.org/2001/XMLSchema#string"/>
  </owl:DatatypeProperty>
  <owl:DatatypeProperty rdf:about="http://example.org/onto/prop/google_network_services_authz_extension_terraform_labels">
    <rdfs:label>terraform_labels</rdfs:label>
    <rdfs:comment>The combination of labels configured directly on the resource
 and default labels configured on the provider.</rdfs:comment>
    <rdfs:domain rdf:resource="http://example.org/onto/class/google_network_services_authz_extension"/>
    <rdfs:range rdf:resource="http://www.w3.org/2001/XMLSchema#string"/>
  </owl:DatatypeProperty>
  <owl:DatatypeProperty rdf:about="http://example.org/onto/prop/google_network_services_authz_extension_timeout">
    <rdfs:label>timeout</rdfs:label>
    <rdfs:comment>Specifies the timeout for each individual message on the stream. The timeout must be between 10-10000 milliseconds.</rdfs:comment>
    <rdfs:domain rdf:resource="http://example.org/onto/class/google_network_services_authz_extension"/>
    <rdfs:range rdf:resource="http://www.w3.org/2001/XMLSchema#string"/>
  </owl:DatatypeProperty>
  <owl:DatatypeProperty rdf:about="http://example.org/onto/prop/google_network_services_authz_extension_update_time">
    <rdfs:label>update_time</rdfs:label>
    <rdfs:comment>The timestamp when the resource was updated.</rdfs:comment>
    <rdfs:domain rdf:resource="http://example.org/onto/class/google_network_services_authz_extension"/>
    <rdfs:range rdf:resource="http://www.w3.org/2001/XMLSchema#string"/>
  </owl:DatatypeProperty>
  <owl:DatatypeProperty rdf:about="http://example.org/onto/prop/google_network_services_authz_extension_wire_format">
    <rdfs:label>wire_format</rdfs:label>
    <rdfs:comment>The format of communication supported by the callout extension. Will be set to EXT_PROC_GRPC by the backend if no value is set. Possible values: ["WIRE_FORMAT_UNSPECIFIED", "EXT_PROC_GRPC"]</rdfs:comment>
    <rdfs:domain rdf:resource="http://example.org/onto/class/google_network_services_authz_extension"/>
    <rdfs:range rdf:resource="http://www.w3.org/2001/XMLSchema#string"/>
  </owl:DatatypeProperty>
  <owl:DatatypeProperty rdf:about="http://example.org/onto/prop/google_network_services_authz_extension_create">
    <rdfs:label>create</rdfs:label>
    <rdfs:domain rdf:resource="http://example.org/onto/class/google_network_services_authz_extension"/>
    <rdfs:range rdf:resource="http://www.w3.org/2001/XMLSchema#string"/>
  </owl:DatatypeProperty>
  <owl:DatatypeProperty rdf:about="http://example.org/onto/prop/google_network_services_authz_extension_delete">
    <rdfs:label>delete</rdfs:label>
    <rdfs:domain rdf:resource="http://example.org/onto/class/google_network_services_authz_extension"/>
    <rdfs:range rdf:resource="http://www.w3.org/2001/XMLSchema#string"/>
  </owl:DatatypeProperty>
  <owl:DatatypeProperty rdf:about="http://example.org/onto/prop/google_network_services_authz_extension_update">
    <rdfs:label>update</rdfs:label>
    <rdfs:domain rdf:resource="http://example.org/onto/class/google_network_services_authz_extension"/>
    <rdfs:range rdf:resource="http://www.w3.org/2001/XMLSchema#string"/>
  </owl:DatatypeProperty>
</rdf:RDF>
