<?xml version="1.0" encoding="UTF-8"?>
<rdf:RDF
  xmlns:rdf="http://www.w3.org/1999/02/22-rdf-syntax-ns#"
  xmlns:rdfs="http://www.w3.org/2000/01/rdf-schema#"
  xmlns:owl="http://www.w3.org/2002/07/owl#"
  xmlns:xsd="http://www.w3.org/2001/XMLSchema#"
  xml:base="http://example.org/onto/">
  <owl:Class rdf:about="http://example.org/onto/class/google_compute_network_endpoint_group">
    <rdfs:label>google_compute_network_endpoint_group</rdfs:label>
    <rdfs:comment>#
#     ***     AUTO GENERATED CODE    ***    Type: MMv1     ***
#
# ----------------------------------------------------------------------------
#
#     This code is generated by Magic Modules using the following:
#
#     Configuration: https:#github.com/GoogleCloudPlatform/magic-modules/tree/main/mmv1/products/compute/NetworkEndpointGroup.yaml
#     Template:      https:#github.com/GoogleCloudPlatform/magic-modules/tree/main/mmv1/templates/terraform/resource.html.markdown.tmpl
#
#     DO NOT EDIT this file directly. Any changes made to this file will be
#     overwritten during the next generation cycle.
#
# ----------------------------------------------------------------------------
subcategory: "Compute Engine"
description: |-
  Network endpoint groups (NEGs) are zonal resources that represent
  collections of IP address and port combinations for GCP resources within a
  single subnet.
---</rdfs:comment>
  </owl:Class>
  <owl:DatatypeProperty rdf:about="http://example.org/onto/prop/google_compute_network_endpoint_group_default_port">
    <rdfs:label>default_port</rdfs:label>
    <rdfs:comment>The default port used if the port number is not specified in the
network endpoint.</rdfs:comment>
    <rdfs:domain rdf:resource="http://example.org/onto/class/google_compute_network_endpoint_group"/>
    <rdfs:range rdf:resource="http://www.w3.org/2001/XMLSchema#string"/>
  </owl:DatatypeProperty>
  <owl:DatatypeProperty rdf:about="http://example.org/onto/prop/google_compute_network_endpoint_group_description">
    <rdfs:label>description</rdfs:label>
    <rdfs:comment>An optional description of this resource. Provide this property when
you create the resource.</rdfs:comment>
    <rdfs:domain rdf:resource="http://example.org/onto/class/google_compute_network_endpoint_group"/>
    <rdfs:range rdf:resource="http://www.w3.org/2001/XMLSchema#string"/>
  </owl:DatatypeProperty>
  <owl:DatatypeProperty rdf:about="http://example.org/onto/prop/google_compute_network_endpoint_group_generated_id">
    <rdfs:label>generated_id</rdfs:label>
    <rdfs:comment>The uniquely generated identifier for the resource. This identifier is defined by the server.</rdfs:comment>
    <rdfs:domain rdf:resource="http://example.org/onto/class/google_compute_network_endpoint_group"/>
    <rdfs:range rdf:resource="http://www.w3.org/2001/XMLSchema#string"/>
  </owl:DatatypeProperty>
  <owl:DatatypeProperty rdf:about="http://example.org/onto/prop/google_compute_network_endpoint_group_id">
    <rdfs:label>id</rdfs:label>
    <rdfs:domain rdf:resource="http://example.org/onto/class/google_compute_network_endpoint_group"/>
    <rdfs:range rdf:resource="http://www.w3.org/2001/XMLSchema#string"/>
  </owl:DatatypeProperty>
  <owl:DatatypeProperty rdf:about="http://example.org/onto/prop/google_compute_network_endpoint_group_name">
    <rdfs:label>name</rdfs:label>
    <rdfs:comment>Name of the resource; provided by the client when the resource is
created. The name must be 1-63 characters long, and comply with
RFC1035. Specifically, the name must be 1-63 characters long and match
the regular expression '[a-z]([-a-z0-9]*[a-z0-9])?' which means the
first character must be a lowercase letter, and all following
characters must be a dash, lowercase letter, or digit, except the last
character, which cannot be a dash.</rdfs:comment>
    <rdfs:domain rdf:resource="http://example.org/onto/class/google_compute_network_endpoint_group"/>
    <rdfs:range rdf:resource="http://www.w3.org/2001/XMLSchema#string"/>
  </owl:DatatypeProperty>
  <owl:DatatypeProperty rdf:about="http://example.org/onto/prop/google_compute_network_endpoint_group_network">
    <rdfs:label>network</rdfs:label>
    <rdfs:comment>The network to which all network endpoints in the NEG belong.
Uses "default" project network if unspecified.</rdfs:comment>
    <rdfs:domain rdf:resource="http://example.org/onto/class/google_compute_network_endpoint_group"/>
    <rdfs:range rdf:resource="http://www.w3.org/2001/XMLSchema#string"/>
  </owl:DatatypeProperty>
  <owl:DatatypeProperty rdf:about="http://example.org/onto/prop/google_compute_network_endpoint_group_network_endpoint_type">
    <rdfs:label>network_endpoint_type</rdfs:label>
    <rdfs:comment>Type of network endpoints in this network endpoint group.
NON_GCP_PRIVATE_IP_PORT is used for hybrid connectivity network
endpoint groups (see https://cloud.google.com/load-balancing/docs/hybrid).
Note that NON_GCP_PRIVATE_IP_PORT can only be used with Backend Services
that 1) have the following load balancing schemes: EXTERNAL, EXTERNAL_MANAGED,
INTERNAL_MANAGED, and INTERNAL_SELF_MANAGED and 2) support the RATE or
CONNECTION balancing modes.

Possible values include: GCE_VM_IP, GCE_VM_IP_PORT, NON_GCP_PRIVATE_IP_PORT, INTERNET_IP_PORT, INTERNET_FQDN_PORT, SERVERLESS, and PRIVATE_SERVICE_CONNECT. Default value: "GCE_VM_IP_PORT" Possible values: ["GCE_VM_IP", "GCE_VM_IP_PORT", "NON_GCP_PRIVATE_IP_PORT", "INTERNET_IP_PORT", "INTERNET_FQDN_PORT", "SERVERLESS", "PRIVATE_SERVICE_CONNECT"]</rdfs:comment>
    <rdfs:domain rdf:resource="http://example.org/onto/class/google_compute_network_endpoint_group"/>
    <rdfs:range rdf:resource="http://www.w3.org/2001/XMLSchema#string"/>
  </owl:DatatypeProperty>
  <owl:DatatypeProperty rdf:about="http://example.org/onto/prop/google_compute_network_endpoint_group_project">
    <rdfs:label>project</rdfs:label>
    <rdfs:domain rdf:resource="http://example.org/onto/class/google_compute_network_endpoint_group"/>
    <rdfs:range rdf:resource="http://www.w3.org/2001/XMLSchema#string"/>
  </owl:DatatypeProperty>
  <owl:DatatypeProperty rdf:about="http://example.org/onto/prop/google_compute_network_endpoint_group_self_link">
    <rdfs:label>self_link</rdfs:label>
    <rdfs:domain rdf:resource="http://example.org/onto/class/google_compute_network_endpoint_group"/>
    <rdfs:range rdf:resource="http://www.w3.org/2001/XMLSchema#string"/>
  </owl:DatatypeProperty>
  <owl:DatatypeProperty rdf:about="http://example.org/onto/prop/google_compute_network_endpoint_group_size">
    <rdfs:label>size</rdfs:label>
    <rdfs:comment>Number of network endpoints in the network endpoint group.</rdfs:comment>
    <rdfs:domain rdf:resource="http://example.org/onto/class/google_compute_network_endpoint_group"/>
    <rdfs:range rdf:resource="http://www.w3.org/2001/XMLSchema#string"/>
  </owl:DatatypeProperty>
  <owl:DatatypeProperty rdf:about="http://example.org/onto/prop/google_compute_network_endpoint_group_subnetwork">
    <rdfs:label>subnetwork</rdfs:label>
    <rdfs:comment>Optional subnetwork to which all network endpoints in the NEG belong.</rdfs:comment>
    <rdfs:domain rdf:resource="http://example.org/onto/class/google_compute_network_endpoint_group"/>
    <rdfs:range rdf:resource="http://www.w3.org/2001/XMLSchema#string"/>
  </owl:DatatypeProperty>
  <owl:DatatypeProperty rdf:about="http://example.org/onto/prop/google_compute_network_endpoint_group_zone">
    <rdfs:label>zone</rdfs:label>
    <rdfs:comment>Zone where the network endpoint group is located.</rdfs:comment>
    <rdfs:domain rdf:resource="http://example.org/onto/class/google_compute_network_endpoint_group"/>
    <rdfs:range rdf:resource="http://www.w3.org/2001/XMLSchema#string"/>
  </owl:DatatypeProperty>
  <owl:DatatypeProperty rdf:about="http://example.org/onto/prop/google_compute_network_endpoint_group_create">
    <rdfs:label>create</rdfs:label>
    <rdfs:domain rdf:resource="http://example.org/onto/class/google_compute_network_endpoint_group"/>
    <rdfs:range rdf:resource="http://www.w3.org/2001/XMLSchema#string"/>
  </owl:DatatypeProperty>
  <owl:DatatypeProperty rdf:about="http://example.org/onto/prop/google_compute_network_endpoint_group_delete">
    <rdfs:label>delete</rdfs:label>
    <rdfs:domain rdf:resource="http://example.org/onto/class/google_compute_network_endpoint_group"/>
    <rdfs:range rdf:resource="http://www.w3.org/2001/XMLSchema#string"/>
  </owl:DatatypeProperty>
</rdf:RDF>
