<?xml version="1.0" encoding="UTF-8"?>
<rdf:RDF
  xmlns:rdf="http://www.w3.org/1999/02/22-rdf-syntax-ns#"
  xmlns:rdfs="http://www.w3.org/2000/01/rdf-schema#"
  xmlns:owl="http://www.w3.org/2002/07/owl#"
  xmlns:xsd="http://www.w3.org/2001/XMLSchema#"
  xml:base="http://example.org/onto/">
  <owl:Class rdf:about="http://example.org/onto/class/google_binary_authorization_attestor">
    <rdfs:label>google_binary_authorization_attestor</rdfs:label>
    <rdfs:comment>#
#     ***     AUTO GENERATED CODE    ***    Type: MMv1     ***
#
# ----------------------------------------------------------------------------
#
#     This code is generated by Magic Modules using the following:
#
#     Configuration: https:#github.com/GoogleCloudPlatform/magic-modules/tree/main/mmv1/products/binaryauthorization/Attestor.yaml
#     Template:      https:#github.com/GoogleCloudPlatform/magic-modules/tree/main/mmv1/templates/terraform/resource.html.markdown.tmpl
#
#     DO NOT EDIT this file directly. Any changes made to this file will be
#     overwritten during the next generation cycle.
#
# ----------------------------------------------------------------------------
subcategory: "Binary Authorization"
description: |-
  An attestor that attests to container image artifacts.
---</rdfs:comment>
  </owl:Class>
  <owl:DatatypeProperty rdf:about="http://example.org/onto/prop/google_binary_authorization_attestor_description">
    <rdfs:label>description</rdfs:label>
    <rdfs:comment>A descriptive comment. This field may be updated. The field may be
displayed in chooser dialogs.</rdfs:comment>
    <rdfs:domain rdf:resource="http://example.org/onto/class/google_binary_authorization_attestor"/>
    <rdfs:range rdf:resource="http://www.w3.org/2001/XMLSchema#string"/>
  </owl:DatatypeProperty>
  <owl:DatatypeProperty rdf:about="http://example.org/onto/prop/google_binary_authorization_attestor_id">
    <rdfs:label>id</rdfs:label>
    <rdfs:domain rdf:resource="http://example.org/onto/class/google_binary_authorization_attestor"/>
    <rdfs:range rdf:resource="http://www.w3.org/2001/XMLSchema#string"/>
  </owl:DatatypeProperty>
  <owl:DatatypeProperty rdf:about="http://example.org/onto/prop/google_binary_authorization_attestor_name">
    <rdfs:label>name</rdfs:label>
    <rdfs:comment>The resource name.</rdfs:comment>
    <rdfs:domain rdf:resource="http://example.org/onto/class/google_binary_authorization_attestor"/>
    <rdfs:range rdf:resource="http://www.w3.org/2001/XMLSchema#string"/>
  </owl:DatatypeProperty>
  <owl:DatatypeProperty rdf:about="http://example.org/onto/prop/google_binary_authorization_attestor_project">
    <rdfs:label>project</rdfs:label>
    <rdfs:domain rdf:resource="http://example.org/onto/class/google_binary_authorization_attestor"/>
    <rdfs:range rdf:resource="http://www.w3.org/2001/XMLSchema#string"/>
  </owl:DatatypeProperty>
  <owl:DatatypeProperty rdf:about="http://example.org/onto/prop/google_binary_authorization_attestor_delegation_service_account_email">
    <rdfs:label>delegation_service_account_email</rdfs:label>
    <rdfs:comment>This field will contain the service account email address that
this Attestor will use as the principal when querying Container
Analysis. Attestor administrators must grant this service account
the IAM role needed to read attestations from the noteReference in
Container Analysis (containeranalysis.notes.occurrences.viewer).
This email address is fixed for the lifetime of the Attestor, but
callers should not make any other assumptions about the service
account email; future versions may use an email based on a
different naming pattern.</rdfs:comment>
    <rdfs:domain rdf:resource="http://example.org/onto/class/google_binary_authorization_attestor"/>
    <rdfs:range rdf:resource="http://www.w3.org/2001/XMLSchema#string"/>
  </owl:DatatypeProperty>
  <owl:DatatypeProperty rdf:about="http://example.org/onto/prop/google_binary_authorization_attestor_note_reference">
    <rdfs:label>note_reference</rdfs:label>
    <rdfs:comment>The resource name of a ATTESTATION_AUTHORITY Note, created by the
user. If the Note is in a different project from the Attestor, it
should be specified in the format 'projects/*/notes/*' (or the legacy
'providers/*/notes/*'). This field may not be updated.
An attestation by this attestor is stored as a Container Analysis
ATTESTATION_AUTHORITY Occurrence that names a container image
and that links to this Note.</rdfs:comment>
    <rdfs:domain rdf:resource="http://example.org/onto/class/google_binary_authorization_attestor"/>
    <rdfs:range rdf:resource="http://www.w3.org/2001/XMLSchema#string"/>
  </owl:DatatypeProperty>
  <owl:DatatypeProperty rdf:about="http://example.org/onto/prop/google_binary_authorization_attestor_ascii_armored_pgp_public_key">
    <rdfs:label>ascii_armored_pgp_public_key</rdfs:label>
    <rdfs:comment>ASCII-armored representation of a PGP public key, as the
entire output by the command
'gpg --export --armor foo@example.com' (either LF or CRLF
line endings). When using this field, id should be left
blank. The BinAuthz API handlers will calculate the ID
and fill it in automatically. BinAuthz computes this ID
as the OpenPGP RFC4880 V4 fingerprint, represented as
upper-case hex. If id is provided by the caller, it will
be overwritten by the API-calculated ID.</rdfs:comment>
    <rdfs:domain rdf:resource="http://example.org/onto/class/google_binary_authorization_attestor"/>
    <rdfs:range rdf:resource="http://www.w3.org/2001/XMLSchema#string"/>
  </owl:DatatypeProperty>
  <owl:DatatypeProperty rdf:about="http://example.org/onto/prop/google_binary_authorization_attestor_comment">
    <rdfs:label>comment</rdfs:label>
    <rdfs:comment>A descriptive comment. This field may be updated.</rdfs:comment>
    <rdfs:domain rdf:resource="http://example.org/onto/class/google_binary_authorization_attestor"/>
    <rdfs:range rdf:resource="http://www.w3.org/2001/XMLSchema#string"/>
  </owl:DatatypeProperty>
  <owl:DatatypeProperty rdf:about="http://example.org/onto/prop/google_binary_authorization_attestor_id">
    <rdfs:label>id</rdfs:label>
    <rdfs:comment>The ID of this public key. Signatures verified by BinAuthz
must include the ID of the public key that can be used to
verify them, and that ID must match the contents of this
field exactly. Additional restrictions on this field can
be imposed based on which public key type is encapsulated.
See the documentation on publicKey cases below for details.</rdfs:comment>
    <rdfs:domain rdf:resource="http://example.org/onto/class/google_binary_authorization_attestor"/>
    <rdfs:range rdf:resource="http://www.w3.org/2001/XMLSchema#string"/>
  </owl:DatatypeProperty>
  <owl:DatatypeProperty rdf:about="http://example.org/onto/prop/google_binary_authorization_attestor_public_key_pem">
    <rdfs:label>public_key_pem</rdfs:label>
    <rdfs:comment>A PEM-encoded public key, as described in
'https://tools.ietf.org/html/rfc7468#section-13'</rdfs:comment>
    <rdfs:domain rdf:resource="http://example.org/onto/class/google_binary_authorization_attestor"/>
    <rdfs:range rdf:resource="http://www.w3.org/2001/XMLSchema#string"/>
  </owl:DatatypeProperty>
  <owl:DatatypeProperty rdf:about="http://example.org/onto/prop/google_binary_authorization_attestor_signature_algorithm">
    <rdfs:label>signature_algorithm</rdfs:label>
    <rdfs:comment>The signature algorithm used to verify a message against
a signature using this key. These signature algorithm must
match the structure and any object identifiers encoded in
publicKeyPem (i.e. this algorithm must match that of the
public key).</rdfs:comment>
    <rdfs:domain rdf:resource="http://example.org/onto/class/google_binary_authorization_attestor"/>
    <rdfs:range rdf:resource="http://www.w3.org/2001/XMLSchema#string"/>
  </owl:DatatypeProperty>
  <owl:DatatypeProperty rdf:about="http://example.org/onto/prop/google_binary_authorization_attestor_create">
    <rdfs:label>create</rdfs:label>
    <rdfs:domain rdf:resource="http://example.org/onto/class/google_binary_authorization_attestor"/>
    <rdfs:range rdf:resource="http://www.w3.org/2001/XMLSchema#string"/>
  </owl:DatatypeProperty>
  <owl:DatatypeProperty rdf:about="http://example.org/onto/prop/google_binary_authorization_attestor_delete">
    <rdfs:label>delete</rdfs:label>
    <rdfs:domain rdf:resource="http://example.org/onto/class/google_binary_authorization_attestor"/>
    <rdfs:range rdf:resource="http://www.w3.org/2001/XMLSchema#string"/>
  </owl:DatatypeProperty>
  <owl:DatatypeProperty rdf:about="http://example.org/onto/prop/google_binary_authorization_attestor_update">
    <rdfs:label>update</rdfs:label>
    <rdfs:domain rdf:resource="http://example.org/onto/class/google_binary_authorization_attestor"/>
    <rdfs:range rdf:resource="http://www.w3.org/2001/XMLSchema#string"/>
  </owl:DatatypeProperty>
</rdf:RDF>
