<?xml version="1.0" encoding="UTF-8"?>
<rdf:RDF
  xmlns:rdf="http://www.w3.org/1999/02/22-rdf-syntax-ns#"
  xmlns:rdfs="http://www.w3.org/2000/01/rdf-schema#"
  xmlns:owl="http://www.w3.org/2002/07/owl#"
  xmlns:xsd="http://www.w3.org/2001/XMLSchema#"
  xml:base="http://example.org/onto/">
  <owl:Class rdf:about="http://example.org/onto/class/google_certificate_manager_dns_authorization">
    <rdfs:label>google_certificate_manager_dns_authorization</rdfs:label>
    <rdfs:comment>#
#     ***     AUTO GENERATED CODE    ***    Type: MMv1     ***
#
# ----------------------------------------------------------------------------
#
#     This code is generated by Magic Modules using the following:
#
#     Configuration: https:#github.com/GoogleCloudPlatform/magic-modules/tree/main/mmv1/products/certificatemanager/DnsAuthorization.yaml
#     Template:      https:#github.com/GoogleCloudPlatform/magic-modules/tree/main/mmv1/templates/terraform/resource.html.markdown.tmpl
#
#     DO NOT EDIT this file directly. Any changes made to this file will be
#     overwritten during the next generation cycle.
#
# ----------------------------------------------------------------------------
subcategory: "Certificate Manager"
description: |-
  DnsAuthorization represents a HTTP-reachable backend for a DnsAuthorization.
---</rdfs:comment>
  </owl:Class>
  <owl:DatatypeProperty rdf:about="http://example.org/onto/prop/google_certificate_manager_dns_authorization_description">
    <rdfs:label>description</rdfs:label>
    <rdfs:comment>A human-readable description of the resource.</rdfs:comment>
    <rdfs:domain rdf:resource="http://example.org/onto/class/google_certificate_manager_dns_authorization"/>
    <rdfs:range rdf:resource="http://www.w3.org/2001/XMLSchema#string"/>
  </owl:DatatypeProperty>
  <owl:DatatypeProperty rdf:about="http://example.org/onto/prop/google_certificate_manager_dns_authorization_dns_resource_record">
    <rdfs:label>dns_resource_record</rdfs:label>
    <rdfs:comment>The structure describing the DNS Resource Record that needs to be added
to DNS configuration for the authorization to be usable by
certificate.</rdfs:comment>
    <rdfs:domain rdf:resource="http://example.org/onto/class/google_certificate_manager_dns_authorization"/>
    <rdfs:range rdf:resource="http://www.w3.org/2001/XMLSchema#string"/>
  </owl:DatatypeProperty>
  <owl:DatatypeProperty rdf:about="http://example.org/onto/prop/google_certificate_manager_dns_authorization_domain">
    <rdfs:label>domain</rdfs:label>
    <rdfs:comment>A domain which is being authorized. A DnsAuthorization resource covers a
single domain and its wildcard, e.g. authorization for "example.com" can
be used to issue certificates for "example.com" and "*.example.com".</rdfs:comment>
    <rdfs:domain rdf:resource="http://example.org/onto/class/google_certificate_manager_dns_authorization"/>
    <rdfs:range rdf:resource="http://www.w3.org/2001/XMLSchema#string"/>
  </owl:DatatypeProperty>
  <owl:DatatypeProperty rdf:about="http://example.org/onto/prop/google_certificate_manager_dns_authorization_effective_labels">
    <rdfs:label>effective_labels</rdfs:label>
    <rdfs:comment>All of labels (key/value pairs) present on the resource in GCP, including the labels configured through Terraform, other clients and services.</rdfs:comment>
    <rdfs:domain rdf:resource="http://example.org/onto/class/google_certificate_manager_dns_authorization"/>
    <rdfs:range rdf:resource="http://www.w3.org/2001/XMLSchema#string"/>
  </owl:DatatypeProperty>
  <owl:DatatypeProperty rdf:about="http://example.org/onto/prop/google_certificate_manager_dns_authorization_id">
    <rdfs:label>id</rdfs:label>
    <rdfs:domain rdf:resource="http://example.org/onto/class/google_certificate_manager_dns_authorization"/>
    <rdfs:range rdf:resource="http://www.w3.org/2001/XMLSchema#string"/>
  </owl:DatatypeProperty>
  <owl:DatatypeProperty rdf:about="http://example.org/onto/prop/google_certificate_manager_dns_authorization_labels">
    <rdfs:label>labels</rdfs:label>
    <rdfs:comment>Set of label tags associated with the DNS Authorization resource.

**Note**: This field is non-authoritative, and will only manage the labels present in your configuration.
Please refer to the field 'effective_labels' for all of the labels present on the resource.</rdfs:comment>
    <rdfs:domain rdf:resource="http://example.org/onto/class/google_certificate_manager_dns_authorization"/>
    <rdfs:range rdf:resource="http://www.w3.org/2001/XMLSchema#string"/>
  </owl:DatatypeProperty>
  <owl:DatatypeProperty rdf:about="http://example.org/onto/prop/google_certificate_manager_dns_authorization_location">
    <rdfs:label>location</rdfs:label>
    <rdfs:comment>The Certificate Manager location. If not specified, "global" is used.</rdfs:comment>
    <rdfs:domain rdf:resource="http://example.org/onto/class/google_certificate_manager_dns_authorization"/>
    <rdfs:range rdf:resource="http://www.w3.org/2001/XMLSchema#string"/>
  </owl:DatatypeProperty>
  <owl:DatatypeProperty rdf:about="http://example.org/onto/prop/google_certificate_manager_dns_authorization_name">
    <rdfs:label>name</rdfs:label>
    <rdfs:comment>Name of the resource; provided by the client when the resource is created.
The name must be 1-64 characters long, and match the regular expression [a-zA-Z][a-zA-Z0-9_-]* which means the first character must be a letter,
and all following characters must be a dash, underscore, letter or digit.</rdfs:comment>
    <rdfs:domain rdf:resource="http://example.org/onto/class/google_certificate_manager_dns_authorization"/>
    <rdfs:range rdf:resource="http://www.w3.org/2001/XMLSchema#string"/>
  </owl:DatatypeProperty>
  <owl:DatatypeProperty rdf:about="http://example.org/onto/prop/google_certificate_manager_dns_authorization_project">
    <rdfs:label>project</rdfs:label>
    <rdfs:domain rdf:resource="http://example.org/onto/class/google_certificate_manager_dns_authorization"/>
    <rdfs:range rdf:resource="http://www.w3.org/2001/XMLSchema#string"/>
  </owl:DatatypeProperty>
  <owl:DatatypeProperty rdf:about="http://example.org/onto/prop/google_certificate_manager_dns_authorization_terraform_labels">
    <rdfs:label>terraform_labels</rdfs:label>
    <rdfs:comment>The combination of labels configured directly on the resource
 and default labels configured on the provider.</rdfs:comment>
    <rdfs:domain rdf:resource="http://example.org/onto/class/google_certificate_manager_dns_authorization"/>
    <rdfs:range rdf:resource="http://www.w3.org/2001/XMLSchema#string"/>
  </owl:DatatypeProperty>
  <owl:DatatypeProperty rdf:about="http://example.org/onto/prop/google_certificate_manager_dns_authorization_type">
    <rdfs:label>type</rdfs:label>
    <rdfs:comment>type of DNS authorization. If unset during the resource creation, FIXED_RECORD will
be used for global resources, and PER_PROJECT_RECORD will be used for other locations.

FIXED_RECORD DNS authorization uses DNS-01 validation method

PER_PROJECT_RECORD DNS authorization allows for independent management
of Google-managed certificates with DNS authorization across multiple
projects. Possible values: ["FIXED_RECORD", "PER_PROJECT_RECORD"]</rdfs:comment>
    <rdfs:domain rdf:resource="http://example.org/onto/class/google_certificate_manager_dns_authorization"/>
    <rdfs:range rdf:resource="http://www.w3.org/2001/XMLSchema#string"/>
  </owl:DatatypeProperty>
  <owl:DatatypeProperty rdf:about="http://example.org/onto/prop/google_certificate_manager_dns_authorization_create">
    <rdfs:label>create</rdfs:label>
    <rdfs:domain rdf:resource="http://example.org/onto/class/google_certificate_manager_dns_authorization"/>
    <rdfs:range rdf:resource="http://www.w3.org/2001/XMLSchema#string"/>
  </owl:DatatypeProperty>
  <owl:DatatypeProperty rdf:about="http://example.org/onto/prop/google_certificate_manager_dns_authorization_delete">
    <rdfs:label>delete</rdfs:label>
    <rdfs:domain rdf:resource="http://example.org/onto/class/google_certificate_manager_dns_authorization"/>
    <rdfs:range rdf:resource="http://www.w3.org/2001/XMLSchema#string"/>
  </owl:DatatypeProperty>
  <owl:DatatypeProperty rdf:about="http://example.org/onto/prop/google_certificate_manager_dns_authorization_update">
    <rdfs:label>update</rdfs:label>
    <rdfs:domain rdf:resource="http://example.org/onto/class/google_certificate_manager_dns_authorization"/>
    <rdfs:range rdf:resource="http://www.w3.org/2001/XMLSchema#string"/>
  </owl:DatatypeProperty>
</rdf:RDF>
