<?xml version="1.0" encoding="UTF-8"?>
<rdf:RDF
  xmlns:rdf="http://www.w3.org/1999/02/22-rdf-syntax-ns#"
  xmlns:rdfs="http://www.w3.org/2000/01/rdf-schema#"
  xmlns:owl="http://www.w3.org/2002/07/owl#"
  xmlns:xsd="http://www.w3.org/2001/XMLSchema#"
  xml:base="http://example.org/onto/">
  <owl:Class rdf:about="http://example.org/onto/class/google_privileged_access_manager_entitlement">
    <rdfs:label>google_privileged_access_manager_entitlement</rdfs:label>
    <rdfs:comment>#
#     ***     AUTO GENERATED CODE    ***    Type: MMv1     ***
#
# ----------------------------------------------------------------------------
#
#     This code is generated by Magic Modules using the following:
#
#     Configuration: https:#github.com/GoogleCloudPlatform/magic-modules/tree/main/mmv1/products/privilegedaccessmanager/Entitlement.yaml
#     Template:      https:#github.com/GoogleCloudPlatform/magic-modules/tree/main/mmv1/templates/terraform/resource.html.markdown.tmpl
#
#     DO NOT EDIT this file directly. Any changes made to this file will be
#     overwritten during the next generation cycle.
#
# ----------------------------------------------------------------------------
subcategory: "Privileged Access Manager"
description: |-
  An Entitlement defines the eligibility of a set of users to obtain a predefined access for some time possibly after going through an approval workflow.
---</rdfs:comment>
  </owl:Class>
  <owl:DatatypeProperty rdf:about="http://example.org/onto/prop/google_privileged_access_manager_entitlement_create_time">
    <rdfs:label>create_time</rdfs:label>
    <rdfs:comment>Output only. Create time stamp. A timestamp in RFC3339 UTC "Zulu" format, with nanosecond resolution and up to nine fractional digits.
Examples: "2014-10-02T15:01:23Z" and "2014-10-02T15:01:23.045123456Z"</rdfs:comment>
    <rdfs:domain rdf:resource="http://example.org/onto/class/google_privileged_access_manager_entitlement"/>
    <rdfs:range rdf:resource="http://www.w3.org/2001/XMLSchema#string"/>
  </owl:DatatypeProperty>
  <owl:DatatypeProperty rdf:about="http://example.org/onto/prop/google_privileged_access_manager_entitlement_entitlement_id">
    <rdfs:label>entitlement_id</rdfs:label>
    <rdfs:comment>The ID to use for this Entitlement. This will become the last part of the resource name.
This value should be 4-63 characters, and valid characters are "[a-z]", "[0-9]", and "-". The first character should be from [a-z].
This value should be unique among all other Entitlements under the specified 'parent'.</rdfs:comment>
    <rdfs:domain rdf:resource="http://example.org/onto/class/google_privileged_access_manager_entitlement"/>
    <rdfs:range rdf:resource="http://www.w3.org/2001/XMLSchema#string"/>
  </owl:DatatypeProperty>
  <owl:DatatypeProperty rdf:about="http://example.org/onto/prop/google_privileged_access_manager_entitlement_etag">
    <rdfs:label>etag</rdfs:label>
    <rdfs:comment>For Resource freshness validation (https://google.aip.dev/154)</rdfs:comment>
    <rdfs:domain rdf:resource="http://example.org/onto/class/google_privileged_access_manager_entitlement"/>
    <rdfs:range rdf:resource="http://www.w3.org/2001/XMLSchema#string"/>
  </owl:DatatypeProperty>
  <owl:DatatypeProperty rdf:about="http://example.org/onto/prop/google_privileged_access_manager_entitlement_id">
    <rdfs:label>id</rdfs:label>
    <rdfs:domain rdf:resource="http://example.org/onto/class/google_privileged_access_manager_entitlement"/>
    <rdfs:range rdf:resource="http://www.w3.org/2001/XMLSchema#string"/>
  </owl:DatatypeProperty>
  <owl:DatatypeProperty rdf:about="http://example.org/onto/prop/google_privileged_access_manager_entitlement_location">
    <rdfs:label>location</rdfs:label>
    <rdfs:comment>The region of the Entitlement resource.</rdfs:comment>
    <rdfs:domain rdf:resource="http://example.org/onto/class/google_privileged_access_manager_entitlement"/>
    <rdfs:range rdf:resource="http://www.w3.org/2001/XMLSchema#string"/>
  </owl:DatatypeProperty>
  <owl:DatatypeProperty rdf:about="http://example.org/onto/prop/google_privileged_access_manager_entitlement_max_request_duration">
    <rdfs:label>max_request_duration</rdfs:label>
    <rdfs:comment>The maximum amount of time for which access would be granted for a request.
A requester can choose to ask for access for less than this duration but never more.
Format: calculate the time in seconds and concatenate it with 's' i.e. 2 hours = "7200s", 45 minutes = "2700s"</rdfs:comment>
    <rdfs:domain rdf:resource="http://example.org/onto/class/google_privileged_access_manager_entitlement"/>
    <rdfs:range rdf:resource="http://www.w3.org/2001/XMLSchema#string"/>
  </owl:DatatypeProperty>
  <owl:DatatypeProperty rdf:about="http://example.org/onto/prop/google_privileged_access_manager_entitlement_name">
    <rdfs:label>name</rdfs:label>
    <rdfs:comment>Output Only. The entitlement's name follows a hierarchical structure, comprising the organization, folder, or project, alongside the region and a unique entitlement ID.
Formats: organizations/{organization-number}/locations/{region}/entitlements/{entitlement-id}, folders/{folder-number}/locations/{region}/entitlements/{entitlement-id}, and projects/{project-id|project-number}/locations/{region}/entitlements/{entitlement-id}.</rdfs:comment>
    <rdfs:domain rdf:resource="http://example.org/onto/class/google_privileged_access_manager_entitlement"/>
    <rdfs:range rdf:resource="http://www.w3.org/2001/XMLSchema#string"/>
  </owl:DatatypeProperty>
  <owl:DatatypeProperty rdf:about="http://example.org/onto/prop/google_privileged_access_manager_entitlement_parent">
    <rdfs:label>parent</rdfs:label>
    <rdfs:comment>Format: projects/{project-id|project-number} or organizations/{organization-number} or folders/{folder-number}</rdfs:comment>
    <rdfs:domain rdf:resource="http://example.org/onto/class/google_privileged_access_manager_entitlement"/>
    <rdfs:range rdf:resource="http://www.w3.org/2001/XMLSchema#string"/>
  </owl:DatatypeProperty>
  <owl:DatatypeProperty rdf:about="http://example.org/onto/prop/google_privileged_access_manager_entitlement_state">
    <rdfs:label>state</rdfs:label>
    <rdfs:comment>Output only. The current state of the Entitlement.</rdfs:comment>
    <rdfs:domain rdf:resource="http://example.org/onto/class/google_privileged_access_manager_entitlement"/>
    <rdfs:range rdf:resource="http://www.w3.org/2001/XMLSchema#string"/>
  </owl:DatatypeProperty>
  <owl:DatatypeProperty rdf:about="http://example.org/onto/prop/google_privileged_access_manager_entitlement_update_time">
    <rdfs:label>update_time</rdfs:label>
    <rdfs:comment>Output only. Update time stamp. A timestamp in RFC3339 UTC "Zulu" format, with nanosecond resolution and up to nine fractional digits.
Examples: "2014-10-02T15:01:23Z" and "2014-10-02T15:01:23.045123456Z".</rdfs:comment>
    <rdfs:domain rdf:resource="http://example.org/onto/class/google_privileged_access_manager_entitlement"/>
    <rdfs:range rdf:resource="http://www.w3.org/2001/XMLSchema#string"/>
  </owl:DatatypeProperty>
  <owl:DatatypeProperty rdf:about="http://example.org/onto/prop/google_privileged_access_manager_entitlement_admin_email_recipients">
    <rdfs:label>admin_email_recipients</rdfs:label>
    <rdfs:comment>Optional. Additional email addresses to be notified when a principal(requester) is granted access.</rdfs:comment>
    <rdfs:domain rdf:resource="http://example.org/onto/class/google_privileged_access_manager_entitlement"/>
    <rdfs:range rdf:resource="http://www.w3.org/2001/XMLSchema#string"/>
  </owl:DatatypeProperty>
  <owl:DatatypeProperty rdf:about="http://example.org/onto/prop/google_privileged_access_manager_entitlement_requester_email_recipients">
    <rdfs:label>requester_email_recipients</rdfs:label>
    <rdfs:comment>Optional. Additional email address to be notified about an eligible entitlement.</rdfs:comment>
    <rdfs:domain rdf:resource="http://example.org/onto/class/google_privileged_access_manager_entitlement"/>
    <rdfs:range rdf:resource="http://www.w3.org/2001/XMLSchema#string"/>
  </owl:DatatypeProperty>
  <owl:DatatypeProperty rdf:about="http://example.org/onto/prop/google_privileged_access_manager_entitlement_require_approver_justification">
    <rdfs:label>require_approver_justification</rdfs:label>
    <rdfs:comment>Optional. Do the approvers need to provide a justification for their actions?</rdfs:comment>
    <rdfs:domain rdf:resource="http://example.org/onto/class/google_privileged_access_manager_entitlement"/>
    <rdfs:range rdf:resource="http://www.w3.org/2001/XMLSchema#string"/>
  </owl:DatatypeProperty>
  <owl:DatatypeProperty rdf:about="http://example.org/onto/prop/google_privileged_access_manager_entitlement_approvals_needed">
    <rdfs:label>approvals_needed</rdfs:label>
    <rdfs:comment>How many users from the above list need to approve.
If there are not enough distinct users in the list above then the workflow
will indefinitely block. Should always be greater than 0. Currently 1 is the only
supported value.</rdfs:comment>
    <rdfs:domain rdf:resource="http://example.org/onto/class/google_privileged_access_manager_entitlement"/>
    <rdfs:range rdf:resource="http://www.w3.org/2001/XMLSchema#string"/>
  </owl:DatatypeProperty>
  <owl:DatatypeProperty rdf:about="http://example.org/onto/prop/google_privileged_access_manager_entitlement_approver_email_recipients">
    <rdfs:label>approver_email_recipients</rdfs:label>
    <rdfs:comment>Optional. Additional email addresses to be notified when a grant is pending approval.</rdfs:comment>
    <rdfs:domain rdf:resource="http://example.org/onto/class/google_privileged_access_manager_entitlement"/>
    <rdfs:range rdf:resource="http://www.w3.org/2001/XMLSchema#string"/>
  </owl:DatatypeProperty>
  <owl:DatatypeProperty rdf:about="http://example.org/onto/prop/google_privileged_access_manager_entitlement_principals">
    <rdfs:label>principals</rdfs:label>
    <rdfs:comment>Users who are being allowed for the operation. Each entry should be a valid v1 IAM Principal Identifier. Format for these is documented at: https://cloud.google.com/iam/docs/principal-identifiers#v1</rdfs:comment>
    <rdfs:domain rdf:resource="http://example.org/onto/class/google_privileged_access_manager_entitlement"/>
    <rdfs:range rdf:resource="http://www.w3.org/2001/XMLSchema#string"/>
  </owl:DatatypeProperty>
  <owl:DatatypeProperty rdf:about="http://example.org/onto/prop/google_privileged_access_manager_entitlement_principals">
    <rdfs:label>principals</rdfs:label>
    <rdfs:comment>Users who are being allowed for the operation. Each entry should be a valid v1 IAM Principal Identifier. Format for these is documented at "https://cloud.google.com/iam/docs/principal-identifiers#v1"</rdfs:comment>
    <rdfs:domain rdf:resource="http://example.org/onto/class/google_privileged_access_manager_entitlement"/>
    <rdfs:range rdf:resource="http://www.w3.org/2001/XMLSchema#string"/>
  </owl:DatatypeProperty>
  <owl:DatatypeProperty rdf:about="http://example.org/onto/prop/google_privileged_access_manager_entitlement_resource">
    <rdfs:label>resource</rdfs:label>
    <rdfs:comment>Name of the resource.</rdfs:comment>
    <rdfs:domain rdf:resource="http://example.org/onto/class/google_privileged_access_manager_entitlement"/>
    <rdfs:range rdf:resource="http://www.w3.org/2001/XMLSchema#string"/>
  </owl:DatatypeProperty>
  <owl:DatatypeProperty rdf:about="http://example.org/onto/prop/google_privileged_access_manager_entitlement_resource_type">
    <rdfs:label>resource_type</rdfs:label>
    <rdfs:comment>The type of this resource.</rdfs:comment>
    <rdfs:domain rdf:resource="http://example.org/onto/class/google_privileged_access_manager_entitlement"/>
    <rdfs:range rdf:resource="http://www.w3.org/2001/XMLSchema#string"/>
  </owl:DatatypeProperty>
  <owl:DatatypeProperty rdf:about="http://example.org/onto/prop/google_privileged_access_manager_entitlement_condition_expression">
    <rdfs:label>condition_expression</rdfs:label>
    <rdfs:comment>The expression field of the IAM condition to be associated with the role. If specified, a user with an active grant for this entitlement would be able to access the resource only if this condition evaluates to true for their request.
https://cloud.google.com/iam/docs/conditions-overview#attributes.</rdfs:comment>
    <rdfs:domain rdf:resource="http://example.org/onto/class/google_privileged_access_manager_entitlement"/>
    <rdfs:range rdf:resource="http://www.w3.org/2001/XMLSchema#string"/>
  </owl:DatatypeProperty>
  <owl:DatatypeProperty rdf:about="http://example.org/onto/prop/google_privileged_access_manager_entitlement_role">
    <rdfs:label>role</rdfs:label>
    <rdfs:comment>IAM role to be granted. https://cloud.google.com/iam/docs/roles-overview.</rdfs:comment>
    <rdfs:domain rdf:resource="http://example.org/onto/class/google_privileged_access_manager_entitlement"/>
    <rdfs:range rdf:resource="http://www.w3.org/2001/XMLSchema#string"/>
  </owl:DatatypeProperty>
  <owl:DatatypeProperty rdf:about="http://example.org/onto/prop/google_privileged_access_manager_entitlement_create">
    <rdfs:label>create</rdfs:label>
    <rdfs:domain rdf:resource="http://example.org/onto/class/google_privileged_access_manager_entitlement"/>
    <rdfs:range rdf:resource="http://www.w3.org/2001/XMLSchema#string"/>
  </owl:DatatypeProperty>
  <owl:DatatypeProperty rdf:about="http://example.org/onto/prop/google_privileged_access_manager_entitlement_delete">
    <rdfs:label>delete</rdfs:label>
    <rdfs:domain rdf:resource="http://example.org/onto/class/google_privileged_access_manager_entitlement"/>
    <rdfs:range rdf:resource="http://www.w3.org/2001/XMLSchema#string"/>
  </owl:DatatypeProperty>
  <owl:DatatypeProperty rdf:about="http://example.org/onto/prop/google_privileged_access_manager_entitlement_update">
    <rdfs:label>update</rdfs:label>
    <rdfs:domain rdf:resource="http://example.org/onto/class/google_privileged_access_manager_entitlement"/>
    <rdfs:range rdf:resource="http://www.w3.org/2001/XMLSchema#string"/>
  </owl:DatatypeProperty>
</rdf:RDF>
