<?xml version="1.0" encoding="UTF-8"?>
<rdf:RDF
  xmlns:rdf="http://www.w3.org/1999/02/22-rdf-syntax-ns#"
  xmlns:rdfs="http://www.w3.org/2000/01/rdf-schema#"
  xmlns:owl="http://www.w3.org/2002/07/owl#"
  xmlns:xsd="http://www.w3.org/2001/XMLSchema#"
  xml:base="http://example.org/onto/">
  <owl:Class rdf:about="http://example.org/onto/class/google_discovery_engine_license_config">
    <rdfs:label>google_discovery_engine_license_config</rdfs:label>
    <rdfs:comment>#
#     ***     AUTO GENERATED CODE    ***    Type: MMv1     ***
#
# ----------------------------------------------------------------------------
#
#     This code is generated by Magic Modules using the following:
#
#     Configuration: https:#github.com/GoogleCloudPlatform/magic-modules/tree/main/mmv1/products/discoveryengine/LicenseConfig.yaml
#     Template:      https:#github.com/GoogleCloudPlatform/magic-modules/tree/main/mmv1/templates/terraform/resource.html.markdown.tmpl
#
#     DO NOT EDIT this file directly. Any changes made to this file will be
#     overwritten during the next generation cycle.
#
# ----------------------------------------------------------------------------
subcategory: "Discovery Engine"
description: |-
  License Configuration.
---</rdfs:comment>
  </owl:Class>
  <owl:DatatypeProperty rdf:about="http://example.org/onto/prop/google_discovery_engine_license_config_auto_renew">
    <rdfs:label>auto_renew</rdfs:label>
    <rdfs:comment>Whether the license config should be auto renewed when it reaches the end date.</rdfs:comment>
    <rdfs:domain rdf:resource="http://example.org/onto/class/google_discovery_engine_license_config"/>
    <rdfs:range rdf:resource="http://www.w3.org/2001/XMLSchema#string"/>
  </owl:DatatypeProperty>
  <owl:DatatypeProperty rdf:about="http://example.org/onto/prop/google_discovery_engine_license_config_free_trial">
    <rdfs:label>free_trial</rdfs:label>
    <rdfs:comment>Whether the license config is for free trial.</rdfs:comment>
    <rdfs:domain rdf:resource="http://example.org/onto/class/google_discovery_engine_license_config"/>
    <rdfs:range rdf:resource="http://www.w3.org/2001/XMLSchema#string"/>
  </owl:DatatypeProperty>
  <owl:DatatypeProperty rdf:about="http://example.org/onto/prop/google_discovery_engine_license_config_id">
    <rdfs:label>id</rdfs:label>
    <rdfs:domain rdf:resource="http://example.org/onto/class/google_discovery_engine_license_config"/>
    <rdfs:range rdf:resource="http://www.w3.org/2001/XMLSchema#string"/>
  </owl:DatatypeProperty>
  <owl:DatatypeProperty rdf:about="http://example.org/onto/prop/google_discovery_engine_license_config_license_config_id">
    <rdfs:label>license_config_id</rdfs:label>
    <rdfs:comment>The unique id of the license config.</rdfs:comment>
    <rdfs:domain rdf:resource="http://example.org/onto/class/google_discovery_engine_license_config"/>
    <rdfs:range rdf:resource="http://www.w3.org/2001/XMLSchema#string"/>
  </owl:DatatypeProperty>
  <owl:DatatypeProperty rdf:about="http://example.org/onto/prop/google_discovery_engine_license_config_license_count">
    <rdfs:label>license_count</rdfs:label>
    <rdfs:comment>Number of licenses purchased.</rdfs:comment>
    <rdfs:domain rdf:resource="http://example.org/onto/class/google_discovery_engine_license_config"/>
    <rdfs:range rdf:resource="http://www.w3.org/2001/XMLSchema#string"/>
  </owl:DatatypeProperty>
  <owl:DatatypeProperty rdf:about="http://example.org/onto/prop/google_discovery_engine_license_config_location">
    <rdfs:label>location</rdfs:label>
    <rdfs:comment>The geographic location where the data store should reside. The value can
only be one of "global", "us" and "eu".</rdfs:comment>
    <rdfs:domain rdf:resource="http://example.org/onto/class/google_discovery_engine_license_config"/>
    <rdfs:range rdf:resource="http://www.w3.org/2001/XMLSchema#string"/>
  </owl:DatatypeProperty>
  <owl:DatatypeProperty rdf:about="http://example.org/onto/prop/google_discovery_engine_license_config_name">
    <rdfs:label>name</rdfs:label>
    <rdfs:comment>The unique full resource name of the license config. Values are of the format
'projects/{project}/locations/{location}/licenseConfigs/{license_config}'.</rdfs:comment>
    <rdfs:domain rdf:resource="http://example.org/onto/class/google_discovery_engine_license_config"/>
    <rdfs:range rdf:resource="http://www.w3.org/2001/XMLSchema#string"/>
  </owl:DatatypeProperty>
  <owl:DatatypeProperty rdf:about="http://example.org/onto/prop/google_discovery_engine_license_config_project">
    <rdfs:label>project</rdfs:label>
    <rdfs:domain rdf:resource="http://example.org/onto/class/google_discovery_engine_license_config"/>
    <rdfs:range rdf:resource="http://www.w3.org/2001/XMLSchema#string"/>
  </owl:DatatypeProperty>
  <owl:DatatypeProperty rdf:about="http://example.org/onto/prop/google_discovery_engine_license_config_subscription_term">
    <rdfs:label>subscription_term</rdfs:label>
    <rdfs:comment>Subscription term. Possible values: ["SUBSCRIPTION_TERM_UNSPECIFIED", "SUBSCRIPTION_TERM_ONE_MONTH", "SUBSCRIPTION_TERM_ONE_YEAR", "SUBSCRIPTION_TERM_THREE_YEARS", "SUBSCRIPTION_TERM_THREE_MONTHS", "SUBSCRIPTION_TERM_FOURTEEN_DAYS", "SUBSCRIPTION_TERM_CUSTOM"]</rdfs:comment>
    <rdfs:domain rdf:resource="http://example.org/onto/class/google_discovery_engine_license_config"/>
    <rdfs:range rdf:resource="http://www.w3.org/2001/XMLSchema#string"/>
  </owl:DatatypeProperty>
  <owl:DatatypeProperty rdf:about="http://example.org/onto/prop/google_discovery_engine_license_config_subscription_tier">
    <rdfs:label>subscription_tier</rdfs:label>
    <rdfs:comment>Subscription tier information for the license config. Possible values: ["SUBSCRIPTION_TIER_UNSPECIFIED", "SUBSCRIPTION_TIER_SEARCH", "SUBSCRIPTION_TIER_SEARCH_AND_ASSISTANT", "SUBSCRIPTION_TIER_NOTEBOOK_LM", "SUBSCRIPTION_TIER_FRONTLINE_WORKER", "SUBSCRIPTION_TIER_AGENTSPACE_STARTER", "SUBSCRIPTION_TIER_AGENTSPACE_BUSINESS", "SUBSCRIPTION_TIER_ENTERPRISE", "SUBSCRIPTION_TIER_EDU", "SUBSCRIPTION_TIER_EDU_PRO"]</rdfs:comment>
    <rdfs:domain rdf:resource="http://example.org/onto/class/google_discovery_engine_license_config"/>
    <rdfs:range rdf:resource="http://www.w3.org/2001/XMLSchema#string"/>
  </owl:DatatypeProperty>
  <owl:DatatypeProperty rdf:about="http://example.org/onto/prop/google_discovery_engine_license_config_day">
    <rdfs:label>day</rdfs:label>
    <rdfs:comment>Day of a month. Must be from 1 to 31 and valid for the year and month, or 0 to specify a year by itself or a year and month where the day isn't significant.</rdfs:comment>
    <rdfs:domain rdf:resource="http://example.org/onto/class/google_discovery_engine_license_config"/>
    <rdfs:range rdf:resource="http://www.w3.org/2001/XMLSchema#string"/>
  </owl:DatatypeProperty>
  <owl:DatatypeProperty rdf:about="http://example.org/onto/prop/google_discovery_engine_license_config_month">
    <rdfs:label>month</rdfs:label>
    <rdfs:comment>Month of a year. Must be from 1 to 12, or 0 to specify a year without a month and day.</rdfs:comment>
    <rdfs:domain rdf:resource="http://example.org/onto/class/google_discovery_engine_license_config"/>
    <rdfs:range rdf:resource="http://www.w3.org/2001/XMLSchema#string"/>
  </owl:DatatypeProperty>
  <owl:DatatypeProperty rdf:about="http://example.org/onto/prop/google_discovery_engine_license_config_year">
    <rdfs:label>year</rdfs:label>
    <rdfs:comment>Year of the date. Must be from 1 to 9999, or 0 to specify a date without a year.</rdfs:comment>
    <rdfs:domain rdf:resource="http://example.org/onto/class/google_discovery_engine_license_config"/>
    <rdfs:range rdf:resource="http://www.w3.org/2001/XMLSchema#string"/>
  </owl:DatatypeProperty>
  <owl:DatatypeProperty rdf:about="http://example.org/onto/prop/google_discovery_engine_license_config_day">
    <rdfs:label>day</rdfs:label>
    <rdfs:comment>Day of a month. Must be from 1 to 31 and valid for the year and month, or 0 to specify a year by itself or a year and month where the day isn't significant.</rdfs:comment>
    <rdfs:domain rdf:resource="http://example.org/onto/class/google_discovery_engine_license_config"/>
    <rdfs:range rdf:resource="http://www.w3.org/2001/XMLSchema#string"/>
  </owl:DatatypeProperty>
  <owl:DatatypeProperty rdf:about="http://example.org/onto/prop/google_discovery_engine_license_config_month">
    <rdfs:label>month</rdfs:label>
    <rdfs:comment>Month of a year. Must be from 1 to 12, or 0 to specify a year without a month and day.</rdfs:comment>
    <rdfs:domain rdf:resource="http://example.org/onto/class/google_discovery_engine_license_config"/>
    <rdfs:range rdf:resource="http://www.w3.org/2001/XMLSchema#string"/>
  </owl:DatatypeProperty>
  <owl:DatatypeProperty rdf:about="http://example.org/onto/prop/google_discovery_engine_license_config_year">
    <rdfs:label>year</rdfs:label>
    <rdfs:comment>Year of the date. Must be from 1 to 9999, or 0 to specify a date without a year.</rdfs:comment>
    <rdfs:domain rdf:resource="http://example.org/onto/class/google_discovery_engine_license_config"/>
    <rdfs:range rdf:resource="http://www.w3.org/2001/XMLSchema#string"/>
  </owl:DatatypeProperty>
  <owl:DatatypeProperty rdf:about="http://example.org/onto/prop/google_discovery_engine_license_config_create">
    <rdfs:label>create</rdfs:label>
    <rdfs:domain rdf:resource="http://example.org/onto/class/google_discovery_engine_license_config"/>
    <rdfs:range rdf:resource="http://www.w3.org/2001/XMLSchema#string"/>
  </owl:DatatypeProperty>
  <owl:DatatypeProperty rdf:about="http://example.org/onto/prop/google_discovery_engine_license_config_delete">
    <rdfs:label>delete</rdfs:label>
    <rdfs:domain rdf:resource="http://example.org/onto/class/google_discovery_engine_license_config"/>
    <rdfs:range rdf:resource="http://www.w3.org/2001/XMLSchema#string"/>
  </owl:DatatypeProperty>
  <owl:DatatypeProperty rdf:about="http://example.org/onto/prop/google_discovery_engine_license_config_update">
    <rdfs:label>update</rdfs:label>
    <rdfs:domain rdf:resource="http://example.org/onto/class/google_discovery_engine_license_config"/>
    <rdfs:range rdf:resource="http://www.w3.org/2001/XMLSchema#string"/>
  </owl:DatatypeProperty>
</rdf:RDF>
