<?xml version="1.0" encoding="UTF-8"?>
<rdf:RDF
  xmlns:rdf="http://www.w3.org/1999/02/22-rdf-syntax-ns#"
  xmlns:rdfs="http://www.w3.org/2000/01/rdf-schema#"
  xmlns:owl="http://www.w3.org/2002/07/owl#"
  xmlns:xsd="http://www.w3.org/2001/XMLSchema#"
  xml:base="http://example.org/onto/">
  <owl:Class rdf:about="http://example.org/onto/class/google_healthcare_hl7_v2_store">
    <rdfs:label>google_healthcare_hl7_v2_store</rdfs:label>
    <rdfs:comment>#
#     ***     AUTO GENERATED CODE    ***    Type: MMv1     ***
#
# ----------------------------------------------------------------------------
#
#     This code is generated by Magic Modules using the following:
#
#     Configuration: https:#github.com/GoogleCloudPlatform/magic-modules/tree/main/mmv1/products/healthcare/Hl7V2Store.yaml
#     Template:      https:#github.com/GoogleCloudPlatform/magic-modules/tree/main/mmv1/templates/terraform/resource.html.markdown.tmpl
#
#     DO NOT EDIT this file directly. Any changes made to this file will be
#     overwritten during the next generation cycle.
#
# ----------------------------------------------------------------------------
subcategory: "Cloud Healthcare"
description: |-
  A Hl7V2Store is a datastore inside a Healthcare dataset that conforms to the FHIR (https://www.
---</rdfs:comment>
  </owl:Class>
  <owl:DatatypeProperty rdf:about="http://example.org/onto/prop/google_healthcare_hl7_v2_store_dataset">
    <rdfs:label>dataset</rdfs:label>
    <rdfs:comment>Identifies the dataset addressed by this request. Must be in the format
'projects/{project}/locations/{location}/datasets/{dataset}'</rdfs:comment>
    <rdfs:domain rdf:resource="http://example.org/onto/class/google_healthcare_hl7_v2_store"/>
    <rdfs:range rdf:resource="http://www.w3.org/2001/XMLSchema#string"/>
  </owl:DatatypeProperty>
  <owl:DatatypeProperty rdf:about="http://example.org/onto/prop/google_healthcare_hl7_v2_store_effective_labels">
    <rdfs:label>effective_labels</rdfs:label>
    <rdfs:comment>All of labels (key/value pairs) present on the resource in GCP, including the labels configured through Terraform, other clients and services.</rdfs:comment>
    <rdfs:domain rdf:resource="http://example.org/onto/class/google_healthcare_hl7_v2_store"/>
    <rdfs:range rdf:resource="http://www.w3.org/2001/XMLSchema#string"/>
  </owl:DatatypeProperty>
  <owl:DatatypeProperty rdf:about="http://example.org/onto/prop/google_healthcare_hl7_v2_store_id">
    <rdfs:label>id</rdfs:label>
    <rdfs:domain rdf:resource="http://example.org/onto/class/google_healthcare_hl7_v2_store"/>
    <rdfs:range rdf:resource="http://www.w3.org/2001/XMLSchema#string"/>
  </owl:DatatypeProperty>
  <owl:DatatypeProperty rdf:about="http://example.org/onto/prop/google_healthcare_hl7_v2_store_labels">
    <rdfs:label>labels</rdfs:label>
    <rdfs:comment>User-supplied key-value pairs used to organize HL7v2 stores.

Label keys must be between 1 and 63 characters long, have a UTF-8 encoding of maximum 128 bytes, and must
conform to the following PCRE regular expression: [\p{Ll}\p{Lo}][\p{Ll}\p{Lo}\p{N}_-]{0,62}

Label values are optional, must be between 1 and 63 characters long, have a UTF-8 encoding of maximum 128
bytes, and must conform to the following PCRE regular expression: [\p{Ll}\p{Lo}\p{N}_-]{0,63}

No more than 64 labels can be associated with a given store.

An object containing a list of "key": value pairs.
Example: { "name": "wrench", "mass": "1.3kg", "count": "3" }.


**Note**: This field is non-authoritative, and will only manage the labels present in your configuration.
Please refer to the field 'effective_labels' for all of the labels present on the resource.</rdfs:comment>
    <rdfs:domain rdf:resource="http://example.org/onto/class/google_healthcare_hl7_v2_store"/>
    <rdfs:range rdf:resource="http://www.w3.org/2001/XMLSchema#string"/>
  </owl:DatatypeProperty>
  <owl:DatatypeProperty rdf:about="http://example.org/onto/prop/google_healthcare_hl7_v2_store_name">
    <rdfs:label>name</rdfs:label>
    <rdfs:comment>The resource name for the Hl7V2Store.

** Changing this property may recreate the Hl7v2 store (removing all data) **</rdfs:comment>
    <rdfs:domain rdf:resource="http://example.org/onto/class/google_healthcare_hl7_v2_store"/>
    <rdfs:range rdf:resource="http://www.w3.org/2001/XMLSchema#string"/>
  </owl:DatatypeProperty>
  <owl:DatatypeProperty rdf:about="http://example.org/onto/prop/google_healthcare_hl7_v2_store_reject_duplicate_message">
    <rdfs:label>reject_duplicate_message</rdfs:label>
    <rdfs:comment>Determines whether duplicate messages are allowed.</rdfs:comment>
    <rdfs:domain rdf:resource="http://example.org/onto/class/google_healthcare_hl7_v2_store"/>
    <rdfs:range rdf:resource="http://www.w3.org/2001/XMLSchema#string"/>
  </owl:DatatypeProperty>
  <owl:DatatypeProperty rdf:about="http://example.org/onto/prop/google_healthcare_hl7_v2_store_self_link">
    <rdfs:label>self_link</rdfs:label>
    <rdfs:comment>The fully qualified name of this dataset</rdfs:comment>
    <rdfs:domain rdf:resource="http://example.org/onto/class/google_healthcare_hl7_v2_store"/>
    <rdfs:range rdf:resource="http://www.w3.org/2001/XMLSchema#string"/>
  </owl:DatatypeProperty>
  <owl:DatatypeProperty rdf:about="http://example.org/onto/prop/google_healthcare_hl7_v2_store_terraform_labels">
    <rdfs:label>terraform_labels</rdfs:label>
    <rdfs:comment>The combination of labels configured directly on the resource
 and default labels configured on the provider.</rdfs:comment>
    <rdfs:domain rdf:resource="http://example.org/onto/class/google_healthcare_hl7_v2_store"/>
    <rdfs:range rdf:resource="http://www.w3.org/2001/XMLSchema#string"/>
  </owl:DatatypeProperty>
  <owl:DatatypeProperty rdf:about="http://example.org/onto/prop/google_healthcare_hl7_v2_store_pubsub_topic">
    <rdfs:label>pubsub_topic</rdfs:label>
    <rdfs:comment>The Cloud Pub/Sub topic that notifications of changes are published on. Supplied by the client.
PubsubMessage.Data will contain the resource name. PubsubMessage.MessageId is the ID of this message.
It is guaranteed to be unique within the topic. PubsubMessage.PublishTime is the time at which the message
was published. Notifications are only sent if the topic is non-empty. Topic names must be scoped to a
project. service-PROJECT_NUMBER@gcp-sa-healthcare.iam.gserviceaccount.com must have publisher permissions on the given
Cloud Pub/Sub topic. Not having adequate permissions will cause the calls that send notifications to fail.</rdfs:comment>
    <rdfs:domain rdf:resource="http://example.org/onto/class/google_healthcare_hl7_v2_store"/>
    <rdfs:range rdf:resource="http://www.w3.org/2001/XMLSchema#string"/>
  </owl:DatatypeProperty>
  <owl:DatatypeProperty rdf:about="http://example.org/onto/prop/google_healthcare_hl7_v2_store_filter">
    <rdfs:label>filter</rdfs:label>
    <rdfs:comment>Restricts notifications sent for messages matching a filter. If this is empty, all messages
are matched. Syntax: https://cloud.google.com/appengine/docs/standard/python/search/query_strings

Fields/functions available for filtering are:

* messageType, from the MSH-9.1 field. For example, NOT messageType = "ADT".
* send_date or sendDate, the YYYY-MM-DD date the message was sent in the dataset's timeZone, from the MSH-7 segment. For example, send_date < "2017-01-02".
* sendTime, the timestamp when the message was sent, using the RFC3339 time format for comparisons, from the MSH-7 segment. For example, sendTime < "2017-01-02T00:00:00-05:00".
* sendFacility, the care center that the message came from, from the MSH-4 segment. For example, sendFacility = "ABC".
* PatientId(value, type), which matches if the message lists a patient having an ID of the given value and type in the PID-2, PID-3, or PID-4 segments. For example, PatientId("123456", "MRN").
* labels.x, a string value of the label with key x as set using the Message.labels map. For example, labels."priority"="high". The operator :* can be used to assert the existence of a label. For example, labels."priority":*.</rdfs:comment>
    <rdfs:domain rdf:resource="http://example.org/onto/class/google_healthcare_hl7_v2_store"/>
    <rdfs:range rdf:resource="http://www.w3.org/2001/XMLSchema#string"/>
  </owl:DatatypeProperty>
  <owl:DatatypeProperty rdf:about="http://example.org/onto/prop/google_healthcare_hl7_v2_store_pubsub_topic">
    <rdfs:label>pubsub_topic</rdfs:label>
    <rdfs:comment>The Cloud Pub/Sub topic that notifications of changes are published on. Supplied by the client.
PubsubMessage.Data will contain the resource name. PubsubMessage.MessageId is the ID of this message.
It is guaranteed to be unique within the topic. PubsubMessage.PublishTime is the time at which the message
was published. Notifications are only sent if the topic is non-empty. Topic names must be scoped to a
project. service-PROJECT_NUMBER@gcp-sa-healthcare.iam.gserviceaccount.com must have publisher permissions on the given
Cloud Pub/Sub topic. Not having adequate permissions will cause the calls that send notifications to fail.

If a notification cannot be published to Cloud Pub/Sub, errors will be logged to Stackdriver</rdfs:comment>
    <rdfs:domain rdf:resource="http://example.org/onto/class/google_healthcare_hl7_v2_store"/>
    <rdfs:range rdf:resource="http://www.w3.org/2001/XMLSchema#string"/>
  </owl:DatatypeProperty>
  <owl:DatatypeProperty rdf:about="http://example.org/onto/prop/google_healthcare_hl7_v2_store_allow_null_header">
    <rdfs:label>allow_null_header</rdfs:label>
    <rdfs:comment>Determines whether messages with no header are allowed.</rdfs:comment>
    <rdfs:domain rdf:resource="http://example.org/onto/class/google_healthcare_hl7_v2_store"/>
    <rdfs:range rdf:resource="http://www.w3.org/2001/XMLSchema#string"/>
  </owl:DatatypeProperty>
  <owl:DatatypeProperty rdf:about="http://example.org/onto/prop/google_healthcare_hl7_v2_store_schema">
    <rdfs:label>schema</rdfs:label>
    <rdfs:comment>JSON encoded string for schemas used to parse messages in this
store if schematized parsing is desired.</rdfs:comment>
    <rdfs:domain rdf:resource="http://example.org/onto/class/google_healthcare_hl7_v2_store"/>
    <rdfs:range rdf:resource="http://www.w3.org/2001/XMLSchema#string"/>
  </owl:DatatypeProperty>
  <owl:DatatypeProperty rdf:about="http://example.org/onto/prop/google_healthcare_hl7_v2_store_segment_terminator">
    <rdfs:label>segment_terminator</rdfs:label>
    <rdfs:comment>Byte(s) to be used as the segment terminator. If this is unset, '\r' will be used as segment terminator.

A base64-encoded string.</rdfs:comment>
    <rdfs:domain rdf:resource="http://example.org/onto/class/google_healthcare_hl7_v2_store"/>
    <rdfs:range rdf:resource="http://www.w3.org/2001/XMLSchema#string"/>
  </owl:DatatypeProperty>
  <owl:DatatypeProperty rdf:about="http://example.org/onto/prop/google_healthcare_hl7_v2_store_version">
    <rdfs:label>version</rdfs:label>
    <rdfs:comment>The version of the unschematized parser to be used when a custom 'schema' is not set. Default value: "V1" Possible values: ["V1", "V2", "V3"]</rdfs:comment>
    <rdfs:domain rdf:resource="http://example.org/onto/class/google_healthcare_hl7_v2_store"/>
    <rdfs:range rdf:resource="http://www.w3.org/2001/XMLSchema#string"/>
  </owl:DatatypeProperty>
  <owl:DatatypeProperty rdf:about="http://example.org/onto/prop/google_healthcare_hl7_v2_store_create">
    <rdfs:label>create</rdfs:label>
    <rdfs:domain rdf:resource="http://example.org/onto/class/google_healthcare_hl7_v2_store"/>
    <rdfs:range rdf:resource="http://www.w3.org/2001/XMLSchema#string"/>
  </owl:DatatypeProperty>
  <owl:DatatypeProperty rdf:about="http://example.org/onto/prop/google_healthcare_hl7_v2_store_delete">
    <rdfs:label>delete</rdfs:label>
    <rdfs:domain rdf:resource="http://example.org/onto/class/google_healthcare_hl7_v2_store"/>
    <rdfs:range rdf:resource="http://www.w3.org/2001/XMLSchema#string"/>
  </owl:DatatypeProperty>
  <owl:DatatypeProperty rdf:about="http://example.org/onto/prop/google_healthcare_hl7_v2_store_update">
    <rdfs:label>update</rdfs:label>
    <rdfs:domain rdf:resource="http://example.org/onto/class/google_healthcare_hl7_v2_store"/>
    <rdfs:range rdf:resource="http://www.w3.org/2001/XMLSchema#string"/>
  </owl:DatatypeProperty>
</rdf:RDF>
