<?xml version="1.0" encoding="UTF-8"?>
<rdf:RDF
  xmlns:rdf="http://www.w3.org/1999/02/22-rdf-syntax-ns#"
  xmlns:rdfs="http://www.w3.org/2000/01/rdf-schema#"
  xmlns:owl="http://www.w3.org/2002/07/owl#"
  xmlns:xsd="http://www.w3.org/2001/XMLSchema#"
  xml:base="http://example.org/onto/">
  <owl:Class rdf:about="http://example.org/onto/class/google_vmwareengine_private_cloud">
    <rdfs:label>google_vmwareengine_private_cloud</rdfs:label>
    <rdfs:comment>#
#     ***     AUTO GENERATED CODE    ***    Type: MMv1     ***
#
# ----------------------------------------------------------------------------
#
#     This code is generated by Magic Modules using the following:
#
#     Configuration: https:#github.com/GoogleCloudPlatform/magic-modules/tree/main/mmv1/products/vmwareengine/PrivateCloud.yaml
#     Template:      https:#github.com/GoogleCloudPlatform/magic-modules/tree/main/mmv1/templates/terraform/resource.html.markdown.tmpl
#
#     DO NOT EDIT this file directly. Any changes made to this file will be
#     overwritten during the next generation cycle.
#
# ----------------------------------------------------------------------------
subcategory: "Cloud VMware Engine"
description: |-
  Represents a private cloud resource.
---</rdfs:comment>
  </owl:Class>
  <owl:DatatypeProperty rdf:about="http://example.org/onto/prop/google_vmwareengine_private_cloud_create_time">
    <rdfs:label>create_time</rdfs:label>
    <rdfs:comment>Creation time of this resource.
A timestamp in RFC3339 UTC "Zulu" format, with nanosecond resolution and up to nine fractional digits.
Examples: "2014-10-02T15:01:23Z" and "2014-10-02T15:01:23.045123456Z".</rdfs:comment>
    <rdfs:domain rdf:resource="http://example.org/onto/class/google_vmwareengine_private_cloud"/>
    <rdfs:range rdf:resource="http://www.w3.org/2001/XMLSchema#string"/>
  </owl:DatatypeProperty>
  <owl:DatatypeProperty rdf:about="http://example.org/onto/prop/google_vmwareengine_private_cloud_delete_time">
    <rdfs:label>delete_time</rdfs:label>
    <rdfs:comment>Time when the resource was scheduled for deletion.
A timestamp in RFC3339 UTC "Zulu" format, with nanosecond resolution and up to nine fractional digits.
Examples: "2014-10-02T15:01:23Z" and "2014-10-02T15:01:23.045123456Z".</rdfs:comment>
    <rdfs:domain rdf:resource="http://example.org/onto/class/google_vmwareengine_private_cloud"/>
    <rdfs:range rdf:resource="http://www.w3.org/2001/XMLSchema#string"/>
  </owl:DatatypeProperty>
  <owl:DatatypeProperty rdf:about="http://example.org/onto/prop/google_vmwareengine_private_cloud_deletion_delay_hours">
    <rdfs:label>deletion_delay_hours</rdfs:label>
    <rdfs:comment>The number of hours to delay this request. You can set this value to an hour between 0 to 8, where setting it to 0 starts the deletion request immediately. If no value is set, a default value is set at the API Level.</rdfs:comment>
    <rdfs:domain rdf:resource="http://example.org/onto/class/google_vmwareengine_private_cloud"/>
    <rdfs:range rdf:resource="http://www.w3.org/2001/XMLSchema#string"/>
  </owl:DatatypeProperty>
  <owl:DatatypeProperty rdf:about="http://example.org/onto/prop/google_vmwareengine_private_cloud_description">
    <rdfs:label>description</rdfs:label>
    <rdfs:comment>User-provided description for this private cloud.</rdfs:comment>
    <rdfs:domain rdf:resource="http://example.org/onto/class/google_vmwareengine_private_cloud"/>
    <rdfs:range rdf:resource="http://www.w3.org/2001/XMLSchema#string"/>
  </owl:DatatypeProperty>
  <owl:DatatypeProperty rdf:about="http://example.org/onto/prop/google_vmwareengine_private_cloud_expire_time">
    <rdfs:label>expire_time</rdfs:label>
    <rdfs:comment>Time when the resource will be irreversibly deleted.
A timestamp in RFC3339 UTC "Zulu" format, with nanosecond resolution and up to nine fractional digits.
Examples: "2014-10-02T15:01:23Z" and "2014-10-02T15:01:23.045123456Z".</rdfs:comment>
    <rdfs:domain rdf:resource="http://example.org/onto/class/google_vmwareengine_private_cloud"/>
    <rdfs:range rdf:resource="http://www.w3.org/2001/XMLSchema#string"/>
  </owl:DatatypeProperty>
  <owl:DatatypeProperty rdf:about="http://example.org/onto/prop/google_vmwareengine_private_cloud_hcx">
    <rdfs:label>hcx</rdfs:label>
    <rdfs:comment>Details about a HCX Cloud Manager appliance.</rdfs:comment>
    <rdfs:domain rdf:resource="http://example.org/onto/class/google_vmwareengine_private_cloud"/>
    <rdfs:range rdf:resource="http://www.w3.org/2001/XMLSchema#string"/>
  </owl:DatatypeProperty>
  <owl:DatatypeProperty rdf:about="http://example.org/onto/prop/google_vmwareengine_private_cloud_id">
    <rdfs:label>id</rdfs:label>
    <rdfs:domain rdf:resource="http://example.org/onto/class/google_vmwareengine_private_cloud"/>
    <rdfs:range rdf:resource="http://www.w3.org/2001/XMLSchema#string"/>
  </owl:DatatypeProperty>
  <owl:DatatypeProperty rdf:about="http://example.org/onto/prop/google_vmwareengine_private_cloud_location">
    <rdfs:label>location</rdfs:label>
    <rdfs:comment>The location where the PrivateCloud should reside.</rdfs:comment>
    <rdfs:domain rdf:resource="http://example.org/onto/class/google_vmwareengine_private_cloud"/>
    <rdfs:range rdf:resource="http://www.w3.org/2001/XMLSchema#string"/>
  </owl:DatatypeProperty>
  <owl:DatatypeProperty rdf:about="http://example.org/onto/prop/google_vmwareengine_private_cloud_name">
    <rdfs:label>name</rdfs:label>
    <rdfs:comment>The ID of the PrivateCloud.</rdfs:comment>
    <rdfs:domain rdf:resource="http://example.org/onto/class/google_vmwareengine_private_cloud"/>
    <rdfs:range rdf:resource="http://www.w3.org/2001/XMLSchema#string"/>
  </owl:DatatypeProperty>
  <owl:DatatypeProperty rdf:about="http://example.org/onto/prop/google_vmwareengine_private_cloud_nsx">
    <rdfs:label>nsx</rdfs:label>
    <rdfs:comment>Details about a NSX Manager appliance.</rdfs:comment>
    <rdfs:domain rdf:resource="http://example.org/onto/class/google_vmwareengine_private_cloud"/>
    <rdfs:range rdf:resource="http://www.w3.org/2001/XMLSchema#string"/>
  </owl:DatatypeProperty>
  <owl:DatatypeProperty rdf:about="http://example.org/onto/prop/google_vmwareengine_private_cloud_project">
    <rdfs:label>project</rdfs:label>
    <rdfs:domain rdf:resource="http://example.org/onto/class/google_vmwareengine_private_cloud"/>
    <rdfs:range rdf:resource="http://www.w3.org/2001/XMLSchema#string"/>
  </owl:DatatypeProperty>
  <owl:DatatypeProperty rdf:about="http://example.org/onto/prop/google_vmwareengine_private_cloud_send_deletion_delay_hours_if_zero">
    <rdfs:label>send_deletion_delay_hours_if_zero</rdfs:label>
    <rdfs:comment>While set true, deletion_delay_hours value will be sent in the request even for zero value of the field. This field is only useful for setting 0 value to the deletion_delay_hours field. It can be used both alone and together with deletion_delay_hours.</rdfs:comment>
    <rdfs:domain rdf:resource="http://example.org/onto/class/google_vmwareengine_private_cloud"/>
    <rdfs:range rdf:resource="http://www.w3.org/2001/XMLSchema#string"/>
  </owl:DatatypeProperty>
  <owl:DatatypeProperty rdf:about="http://example.org/onto/prop/google_vmwareengine_private_cloud_state">
    <rdfs:label>state</rdfs:label>
    <rdfs:comment>State of the resource. New values may be added to this enum when appropriate.</rdfs:comment>
    <rdfs:domain rdf:resource="http://example.org/onto/class/google_vmwareengine_private_cloud"/>
    <rdfs:range rdf:resource="http://www.w3.org/2001/XMLSchema#string"/>
  </owl:DatatypeProperty>
  <owl:DatatypeProperty rdf:about="http://example.org/onto/prop/google_vmwareengine_private_cloud_type">
    <rdfs:label>type</rdfs:label>
    <rdfs:comment>Initial type of the private cloud. Possible values: ["STANDARD", "TIME_LIMITED", "STRETCHED"]</rdfs:comment>
    <rdfs:domain rdf:resource="http://example.org/onto/class/google_vmwareengine_private_cloud"/>
    <rdfs:range rdf:resource="http://www.w3.org/2001/XMLSchema#string"/>
  </owl:DatatypeProperty>
  <owl:DatatypeProperty rdf:about="http://example.org/onto/prop/google_vmwareengine_private_cloud_uid">
    <rdfs:label>uid</rdfs:label>
    <rdfs:comment>System-generated unique identifier for the resource.</rdfs:comment>
    <rdfs:domain rdf:resource="http://example.org/onto/class/google_vmwareengine_private_cloud"/>
    <rdfs:range rdf:resource="http://www.w3.org/2001/XMLSchema#string"/>
  </owl:DatatypeProperty>
  <owl:DatatypeProperty rdf:about="http://example.org/onto/prop/google_vmwareengine_private_cloud_update_time">
    <rdfs:label>update_time</rdfs:label>
    <rdfs:comment>Last update time of this resource.
A timestamp in RFC3339 UTC "Zulu" format, with nanosecond resolution and up to nine fractional digits.
Examples: "2014-10-02T15:01:23Z" and "2014-10-02T15:01:23.045123456Z".</rdfs:comment>
    <rdfs:domain rdf:resource="http://example.org/onto/class/google_vmwareengine_private_cloud"/>
    <rdfs:range rdf:resource="http://www.w3.org/2001/XMLSchema#string"/>
  </owl:DatatypeProperty>
  <owl:DatatypeProperty rdf:about="http://example.org/onto/prop/google_vmwareengine_private_cloud_vcenter">
    <rdfs:label>vcenter</rdfs:label>
    <rdfs:comment>Details about a vCenter Server management appliance.</rdfs:comment>
    <rdfs:domain rdf:resource="http://example.org/onto/class/google_vmwareengine_private_cloud"/>
    <rdfs:range rdf:resource="http://www.w3.org/2001/XMLSchema#string"/>
  </owl:DatatypeProperty>
  <owl:DatatypeProperty rdf:about="http://example.org/onto/prop/google_vmwareengine_private_cloud_cluster_id">
    <rdfs:label>cluster_id</rdfs:label>
    <rdfs:comment>The user-provided identifier of the new Cluster. The identifier must meet the following requirements:
  * Only contains 1-63 alphanumeric characters and hyphens
  * Begins with an alphabetical character
  * Ends with a non-hyphen character
  * Not formatted as a UUID
  * Complies with RFC 1034 (https://datatracker.ietf.org/doc/html/rfc1034) (section 3.5)</rdfs:comment>
    <rdfs:domain rdf:resource="http://example.org/onto/class/google_vmwareengine_private_cloud"/>
    <rdfs:range rdf:resource="http://www.w3.org/2001/XMLSchema#string"/>
  </owl:DatatypeProperty>
  <owl:DatatypeProperty rdf:about="http://example.org/onto/prop/google_vmwareengine_private_cloud_cool_down_period">
    <rdfs:label>cool_down_period</rdfs:label>
    <rdfs:comment>The minimum duration between consecutive autoscale operations.
It starts once addition or removal of nodes is fully completed.
Minimum cool down period is 30m.
Cool down period must be in whole minutes (for example, 30m, 31m, 50m).
Mandatory for successful addition of autoscaling settings in cluster.</rdfs:comment>
    <rdfs:domain rdf:resource="http://example.org/onto/class/google_vmwareengine_private_cloud"/>
    <rdfs:range rdf:resource="http://www.w3.org/2001/XMLSchema#string"/>
  </owl:DatatypeProperty>
  <owl:DatatypeProperty rdf:about="http://example.org/onto/prop/google_vmwareengine_private_cloud_max_cluster_node_count">
    <rdfs:label>max_cluster_node_count</rdfs:label>
    <rdfs:comment>Maximum number of nodes of any type in a cluster.
Mandatory for successful addition of autoscaling settings in cluster.</rdfs:comment>
    <rdfs:domain rdf:resource="http://example.org/onto/class/google_vmwareengine_private_cloud"/>
    <rdfs:range rdf:resource="http://www.w3.org/2001/XMLSchema#string"/>
  </owl:DatatypeProperty>
  <owl:DatatypeProperty rdf:about="http://example.org/onto/prop/google_vmwareengine_private_cloud_min_cluster_node_count">
    <rdfs:label>min_cluster_node_count</rdfs:label>
    <rdfs:comment>Minimum number of nodes of any type in a cluster.
Mandatory for successful addition of autoscaling settings in cluster.</rdfs:comment>
    <rdfs:domain rdf:resource="http://example.org/onto/class/google_vmwareengine_private_cloud"/>
    <rdfs:range rdf:resource="http://www.w3.org/2001/XMLSchema#string"/>
  </owl:DatatypeProperty>
  <owl:DatatypeProperty rdf:about="http://example.org/onto/prop/google_vmwareengine_private_cloud_autoscale_policy_id">
    <rdfs:label>autoscale_policy_id</rdfs:label>
    <rdfs:domain rdf:resource="http://example.org/onto/class/google_vmwareengine_private_cloud"/>
    <rdfs:range rdf:resource="http://www.w3.org/2001/XMLSchema#string"/>
  </owl:DatatypeProperty>
  <owl:DatatypeProperty rdf:about="http://example.org/onto/prop/google_vmwareengine_private_cloud_node_type_id">
    <rdfs:label>node_type_id</rdfs:label>
    <rdfs:comment>The canonical identifier of the node type to add or remove.</rdfs:comment>
    <rdfs:domain rdf:resource="http://example.org/onto/class/google_vmwareengine_private_cloud"/>
    <rdfs:range rdf:resource="http://www.w3.org/2001/XMLSchema#string"/>
  </owl:DatatypeProperty>
  <owl:DatatypeProperty rdf:about="http://example.org/onto/prop/google_vmwareengine_private_cloud_scale_out_size">
    <rdfs:label>scale_out_size</rdfs:label>
    <rdfs:comment>Number of nodes to add to a cluster during a scale-out operation.
Must be divisible by 2 for stretched clusters.</rdfs:comment>
    <rdfs:domain rdf:resource="http://example.org/onto/class/google_vmwareengine_private_cloud"/>
    <rdfs:range rdf:resource="http://www.w3.org/2001/XMLSchema#string"/>
  </owl:DatatypeProperty>
  <owl:DatatypeProperty rdf:about="http://example.org/onto/prop/google_vmwareengine_private_cloud_scale_in">
    <rdfs:label>scale_in</rdfs:label>
    <rdfs:comment>The utilization triggering the scale-in operation in percent.</rdfs:comment>
    <rdfs:domain rdf:resource="http://example.org/onto/class/google_vmwareengine_private_cloud"/>
    <rdfs:range rdf:resource="http://www.w3.org/2001/XMLSchema#string"/>
  </owl:DatatypeProperty>
  <owl:DatatypeProperty rdf:about="http://example.org/onto/prop/google_vmwareengine_private_cloud_scale_out">
    <rdfs:label>scale_out</rdfs:label>
    <rdfs:comment>The utilization triggering the scale-out operation in percent.</rdfs:comment>
    <rdfs:domain rdf:resource="http://example.org/onto/class/google_vmwareengine_private_cloud"/>
    <rdfs:range rdf:resource="http://www.w3.org/2001/XMLSchema#string"/>
  </owl:DatatypeProperty>
  <owl:DatatypeProperty rdf:about="http://example.org/onto/prop/google_vmwareengine_private_cloud_scale_in">
    <rdfs:label>scale_in</rdfs:label>
    <rdfs:comment>The utilization triggering the scale-in operation in percent.</rdfs:comment>
    <rdfs:domain rdf:resource="http://example.org/onto/class/google_vmwareengine_private_cloud"/>
    <rdfs:range rdf:resource="http://www.w3.org/2001/XMLSchema#string"/>
  </owl:DatatypeProperty>
  <owl:DatatypeProperty rdf:about="http://example.org/onto/prop/google_vmwareengine_private_cloud_scale_out">
    <rdfs:label>scale_out</rdfs:label>
    <rdfs:comment>The utilization triggering the scale-out operation in percent.</rdfs:comment>
    <rdfs:domain rdf:resource="http://example.org/onto/class/google_vmwareengine_private_cloud"/>
    <rdfs:range rdf:resource="http://www.w3.org/2001/XMLSchema#string"/>
  </owl:DatatypeProperty>
  <owl:DatatypeProperty rdf:about="http://example.org/onto/prop/google_vmwareengine_private_cloud_scale_in">
    <rdfs:label>scale_in</rdfs:label>
    <rdfs:comment>The utilization triggering the scale-in operation in percent.</rdfs:comment>
    <rdfs:domain rdf:resource="http://example.org/onto/class/google_vmwareengine_private_cloud"/>
    <rdfs:range rdf:resource="http://www.w3.org/2001/XMLSchema#string"/>
  </owl:DatatypeProperty>
  <owl:DatatypeProperty rdf:about="http://example.org/onto/prop/google_vmwareengine_private_cloud_scale_out">
    <rdfs:label>scale_out</rdfs:label>
    <rdfs:comment>The utilization triggering the scale-out operation in percent.</rdfs:comment>
    <rdfs:domain rdf:resource="http://example.org/onto/class/google_vmwareengine_private_cloud"/>
    <rdfs:range rdf:resource="http://www.w3.org/2001/XMLSchema#string"/>
  </owl:DatatypeProperty>
  <owl:DatatypeProperty rdf:about="http://example.org/onto/prop/google_vmwareengine_private_cloud_custom_core_count">
    <rdfs:label>custom_core_count</rdfs:label>
    <rdfs:comment>Customized number of cores available to each node of the type.
This number must always be one of 'nodeType.availableCustomCoreCounts'.
If zero is provided max value from 'nodeType.availableCustomCoreCounts' will be used.
This cannot be changed once the PrivateCloud is created.</rdfs:comment>
    <rdfs:domain rdf:resource="http://example.org/onto/class/google_vmwareengine_private_cloud"/>
    <rdfs:range rdf:resource="http://www.w3.org/2001/XMLSchema#string"/>
  </owl:DatatypeProperty>
  <owl:DatatypeProperty rdf:about="http://example.org/onto/prop/google_vmwareengine_private_cloud_node_count">
    <rdfs:label>node_count</rdfs:label>
    <rdfs:comment>The number of nodes of this type in the cluster.</rdfs:comment>
    <rdfs:domain rdf:resource="http://example.org/onto/class/google_vmwareengine_private_cloud"/>
    <rdfs:range rdf:resource="http://www.w3.org/2001/XMLSchema#string"/>
  </owl:DatatypeProperty>
  <owl:DatatypeProperty rdf:about="http://example.org/onto/prop/google_vmwareengine_private_cloud_node_type_id">
    <rdfs:label>node_type_id</rdfs:label>
    <rdfs:domain rdf:resource="http://example.org/onto/class/google_vmwareengine_private_cloud"/>
    <rdfs:range rdf:resource="http://www.w3.org/2001/XMLSchema#string"/>
  </owl:DatatypeProperty>
  <owl:DatatypeProperty rdf:about="http://example.org/onto/prop/google_vmwareengine_private_cloud_preferred_location">
    <rdfs:label>preferred_location</rdfs:label>
    <rdfs:comment>Zone that will remain operational when connection between the two zones is lost.
Specify the zone in the following format: projects/{project}/locations/{location}.</rdfs:comment>
    <rdfs:domain rdf:resource="http://example.org/onto/class/google_vmwareengine_private_cloud"/>
    <rdfs:range rdf:resource="http://www.w3.org/2001/XMLSchema#string"/>
  </owl:DatatypeProperty>
  <owl:DatatypeProperty rdf:about="http://example.org/onto/prop/google_vmwareengine_private_cloud_secondary_location">
    <rdfs:label>secondary_location</rdfs:label>
    <rdfs:comment>Additional zone for a higher level of availability and load balancing.
Specify the zone in the following format: projects/{project}/locations/{location}.</rdfs:comment>
    <rdfs:domain rdf:resource="http://example.org/onto/class/google_vmwareengine_private_cloud"/>
    <rdfs:range rdf:resource="http://www.w3.org/2001/XMLSchema#string"/>
  </owl:DatatypeProperty>
  <owl:DatatypeProperty rdf:about="http://example.org/onto/prop/google_vmwareengine_private_cloud_dns_server_ip">
    <rdfs:label>dns_server_ip</rdfs:label>
    <rdfs:comment>DNS Server IP of the Private Cloud.</rdfs:comment>
    <rdfs:domain rdf:resource="http://example.org/onto/class/google_vmwareengine_private_cloud"/>
    <rdfs:range rdf:resource="http://www.w3.org/2001/XMLSchema#string"/>
  </owl:DatatypeProperty>
  <owl:DatatypeProperty rdf:about="http://example.org/onto/prop/google_vmwareengine_private_cloud_management_cidr">
    <rdfs:label>management_cidr</rdfs:label>
    <rdfs:comment>Management CIDR used by VMware management appliances.</rdfs:comment>
    <rdfs:domain rdf:resource="http://example.org/onto/class/google_vmwareengine_private_cloud"/>
    <rdfs:range rdf:resource="http://www.w3.org/2001/XMLSchema#string"/>
  </owl:DatatypeProperty>
  <owl:DatatypeProperty rdf:about="http://example.org/onto/prop/google_vmwareengine_private_cloud_management_ip_address_layout_version">
    <rdfs:label>management_ip_address_layout_version</rdfs:label>
    <rdfs:comment>The IP address layout version of the management IP address range.
Possible versions include:
* managementIpAddressLayoutVersion=1: Indicates the legacy IP address layout used by some existing private clouds. This is no longer supported for new private clouds
as it does not support all features.
* managementIpAddressLayoutVersion=2: Indicates the latest IP address layout
used by all newly created private clouds. This version supports all current features.</rdfs:comment>
    <rdfs:domain rdf:resource="http://example.org/onto/class/google_vmwareengine_private_cloud"/>
    <rdfs:range rdf:resource="http://www.w3.org/2001/XMLSchema#string"/>
  </owl:DatatypeProperty>
  <owl:DatatypeProperty rdf:about="http://example.org/onto/prop/google_vmwareengine_private_cloud_vmware_engine_network">
    <rdfs:label>vmware_engine_network</rdfs:label>
    <rdfs:comment>The relative resource name of the VMware Engine network attached to the private cloud.
Specify the name in the following form: projects/{project}/locations/{location}/vmwareEngineNetworks/{vmwareEngineNetworkId}
where {project} can either be a project number or a project ID.</rdfs:comment>
    <rdfs:domain rdf:resource="http://example.org/onto/class/google_vmwareengine_private_cloud"/>
    <rdfs:range rdf:resource="http://www.w3.org/2001/XMLSchema#string"/>
  </owl:DatatypeProperty>
  <owl:DatatypeProperty rdf:about="http://example.org/onto/prop/google_vmwareengine_private_cloud_vmware_engine_network_canonical">
    <rdfs:label>vmware_engine_network_canonical</rdfs:label>
    <rdfs:comment>The canonical name of the VMware Engine network in
the form: projects/{project_number}/locations/{location}/vmwareEngineNetworks/{vmwareEngineNetworkId}</rdfs:comment>
    <rdfs:domain rdf:resource="http://example.org/onto/class/google_vmwareengine_private_cloud"/>
    <rdfs:range rdf:resource="http://www.w3.org/2001/XMLSchema#string"/>
  </owl:DatatypeProperty>
  <owl:DatatypeProperty rdf:about="http://example.org/onto/prop/google_vmwareengine_private_cloud_create">
    <rdfs:label>create</rdfs:label>
    <rdfs:domain rdf:resource="http://example.org/onto/class/google_vmwareengine_private_cloud"/>
    <rdfs:range rdf:resource="http://www.w3.org/2001/XMLSchema#string"/>
  </owl:DatatypeProperty>
  <owl:DatatypeProperty rdf:about="http://example.org/onto/prop/google_vmwareengine_private_cloud_delete">
    <rdfs:label>delete</rdfs:label>
    <rdfs:domain rdf:resource="http://example.org/onto/class/google_vmwareengine_private_cloud"/>
    <rdfs:range rdf:resource="http://www.w3.org/2001/XMLSchema#string"/>
  </owl:DatatypeProperty>
  <owl:DatatypeProperty rdf:about="http://example.org/onto/prop/google_vmwareengine_private_cloud_update">
    <rdfs:label>update</rdfs:label>
    <rdfs:domain rdf:resource="http://example.org/onto/class/google_vmwareengine_private_cloud"/>
    <rdfs:range rdf:resource="http://www.w3.org/2001/XMLSchema#string"/>
  </owl:DatatypeProperty>
</rdf:RDF>
