<?xml version="1.0" encoding="UTF-8"?>
<rdf:RDF
  xmlns:rdf="http://www.w3.org/1999/02/22-rdf-syntax-ns#"
  xmlns:rdfs="http://www.w3.org/2000/01/rdf-schema#"
  xmlns:owl="http://www.w3.org/2002/07/owl#"
  xmlns:xsd="http://www.w3.org/2001/XMLSchema#"
  xml:base="http://example.org/onto/">
  <owl:Class rdf:about="http://example.org/onto/class/google_healthcare_consent_store">
    <rdfs:label>google_healthcare_consent_store</rdfs:label>
    <rdfs:comment>#
#     ***     AUTO GENERATED CODE    ***    Type: MMv1     ***
#
# ----------------------------------------------------------------------------
#
#     This code is generated by Magic Modules using the following:
#
#     Configuration: https:#github.com/GoogleCloudPlatform/magic-modules/tree/main/mmv1/products/healthcare/ConsentStore.yaml
#     Template:      https:#github.com/GoogleCloudPlatform/magic-modules/tree/main/mmv1/templates/terraform/resource.html.markdown.tmpl
#
#     DO NOT EDIT this file directly. Any changes made to this file will be
#     overwritten during the next generation cycle.
#
# ----------------------------------------------------------------------------
subcategory: "Cloud Healthcare"
description: |-
  The Consent Management API is a tool for tracking user consents and the documentation associated with the consents.
---</rdfs:comment>
  </owl:Class>
  <owl:DatatypeProperty rdf:about="http://example.org/onto/prop/google_healthcare_consent_store_dataset">
    <rdfs:label>dataset</rdfs:label>
    <rdfs:comment>Identifies the dataset addressed by this request. Must be in the format
'projects/{project}/locations/{location}/datasets/{dataset}'</rdfs:comment>
    <rdfs:domain rdf:resource="http://example.org/onto/class/google_healthcare_consent_store"/>
    <rdfs:range rdf:resource="http://www.w3.org/2001/XMLSchema#string"/>
  </owl:DatatypeProperty>
  <owl:DatatypeProperty rdf:about="http://example.org/onto/prop/google_healthcare_consent_store_default_consent_ttl">
    <rdfs:label>default_consent_ttl</rdfs:label>
    <rdfs:comment>Default time to live for consents in this store. Must be at least 24 hours. Updating this field will not affect the expiration time of existing consents.

A duration in seconds with up to nine fractional digits, terminated by 's'. Example: "3.5s".</rdfs:comment>
    <rdfs:domain rdf:resource="http://example.org/onto/class/google_healthcare_consent_store"/>
    <rdfs:range rdf:resource="http://www.w3.org/2001/XMLSchema#string"/>
  </owl:DatatypeProperty>
  <owl:DatatypeProperty rdf:about="http://example.org/onto/prop/google_healthcare_consent_store_effective_labels">
    <rdfs:label>effective_labels</rdfs:label>
    <rdfs:comment>All of labels (key/value pairs) present on the resource in GCP, including the labels configured through Terraform, other clients and services.</rdfs:comment>
    <rdfs:domain rdf:resource="http://example.org/onto/class/google_healthcare_consent_store"/>
    <rdfs:range rdf:resource="http://www.w3.org/2001/XMLSchema#string"/>
  </owl:DatatypeProperty>
  <owl:DatatypeProperty rdf:about="http://example.org/onto/prop/google_healthcare_consent_store_enable_consent_create_on_update">
    <rdfs:label>enable_consent_create_on_update</rdfs:label>
    <rdfs:comment>If true, [consents.patch] [google.cloud.healthcare.v1.consent.UpdateConsent] creates the consent if it does not already exist.</rdfs:comment>
    <rdfs:domain rdf:resource="http://example.org/onto/class/google_healthcare_consent_store"/>
    <rdfs:range rdf:resource="http://www.w3.org/2001/XMLSchema#string"/>
  </owl:DatatypeProperty>
  <owl:DatatypeProperty rdf:about="http://example.org/onto/prop/google_healthcare_consent_store_id">
    <rdfs:label>id</rdfs:label>
    <rdfs:domain rdf:resource="http://example.org/onto/class/google_healthcare_consent_store"/>
    <rdfs:range rdf:resource="http://www.w3.org/2001/XMLSchema#string"/>
  </owl:DatatypeProperty>
  <owl:DatatypeProperty rdf:about="http://example.org/onto/prop/google_healthcare_consent_store_labels">
    <rdfs:label>labels</rdfs:label>
    <rdfs:comment>User-supplied key-value pairs used to organize Consent stores.

Label keys must be between 1 and 63 characters long, have a UTF-8 encoding of maximum 128 bytes, and must
conform to the following PCRE regular expression: '[\p{Ll}\p{Lo}][\p{Ll}\p{Lo}\p{N}_-]{0,62}'

Label values are optional, must be between 1 and 63 characters long, have a UTF-8 encoding of maximum 128
bytes, and must conform to the following PCRE regular expression: '[\p{Ll}\p{Lo}\p{N}_-]{0,63}'

No more than 64 labels can be associated with a given store.

An object containing a list of "key": value pairs.
Example: { "name": "wrench", "mass": "1.3kg", "count": "3" }.


**Note**: This field is non-authoritative, and will only manage the labels present in your configuration.
Please refer to the field 'effective_labels' for all of the labels present on the resource.</rdfs:comment>
    <rdfs:domain rdf:resource="http://example.org/onto/class/google_healthcare_consent_store"/>
    <rdfs:range rdf:resource="http://www.w3.org/2001/XMLSchema#string"/>
  </owl:DatatypeProperty>
  <owl:DatatypeProperty rdf:about="http://example.org/onto/prop/google_healthcare_consent_store_name">
    <rdfs:label>name</rdfs:label>
    <rdfs:comment>The name of this ConsentStore, for example:
"consent1"</rdfs:comment>
    <rdfs:domain rdf:resource="http://example.org/onto/class/google_healthcare_consent_store"/>
    <rdfs:range rdf:resource="http://www.w3.org/2001/XMLSchema#string"/>
  </owl:DatatypeProperty>
  <owl:DatatypeProperty rdf:about="http://example.org/onto/prop/google_healthcare_consent_store_terraform_labels">
    <rdfs:label>terraform_labels</rdfs:label>
    <rdfs:comment>The combination of labels configured directly on the resource
 and default labels configured on the provider.</rdfs:comment>
    <rdfs:domain rdf:resource="http://example.org/onto/class/google_healthcare_consent_store"/>
    <rdfs:range rdf:resource="http://www.w3.org/2001/XMLSchema#string"/>
  </owl:DatatypeProperty>
  <owl:DatatypeProperty rdf:about="http://example.org/onto/prop/google_healthcare_consent_store_create">
    <rdfs:label>create</rdfs:label>
    <rdfs:domain rdf:resource="http://example.org/onto/class/google_healthcare_consent_store"/>
    <rdfs:range rdf:resource="http://www.w3.org/2001/XMLSchema#string"/>
  </owl:DatatypeProperty>
  <owl:DatatypeProperty rdf:about="http://example.org/onto/prop/google_healthcare_consent_store_delete">
    <rdfs:label>delete</rdfs:label>
    <rdfs:domain rdf:resource="http://example.org/onto/class/google_healthcare_consent_store"/>
    <rdfs:range rdf:resource="http://www.w3.org/2001/XMLSchema#string"/>
  </owl:DatatypeProperty>
  <owl:DatatypeProperty rdf:about="http://example.org/onto/prop/google_healthcare_consent_store_update">
    <rdfs:label>update</rdfs:label>
    <rdfs:domain rdf:resource="http://example.org/onto/class/google_healthcare_consent_store"/>
    <rdfs:range rdf:resource="http://www.w3.org/2001/XMLSchema#string"/>
  </owl:DatatypeProperty>
</rdf:RDF>
