<?xml version="1.0" encoding="UTF-8"?>
<rdf:RDF
  xmlns:rdf="http://www.w3.org/1999/02/22-rdf-syntax-ns#"
  xmlns:rdfs="http://www.w3.org/2000/01/rdf-schema#"
  xmlns:owl="http://www.w3.org/2002/07/owl#"
  xmlns:xsd="http://www.w3.org/2001/XMLSchema#"
  xml:base="http://example.org/onto/">
  <owl:Class rdf:about="http://example.org/onto/class/google_vpc_access_connector">
    <rdfs:label>google_vpc_access_connector</rdfs:label>
    <rdfs:comment>#
#     ***     AUTO GENERATED CODE    ***    Type: MMv1     ***
#
# ----------------------------------------------------------------------------
#
#     This code is generated by Magic Modules using the following:
#
#     Configuration: https:#github.com/GoogleCloudPlatform/magic-modules/tree/main/mmv1/products/vpcaccess/Connector.yaml
#     Template:      https:#github.com/GoogleCloudPlatform/magic-modules/tree/main/mmv1/templates/terraform/resource.html.markdown.tmpl
#
#     DO NOT EDIT this file directly. Any changes made to this file will be
#     overwritten during the next generation cycle.
#
# ----------------------------------------------------------------------------
subcategory: "Serverless VPC Access"
description: |-
  Serverless VPC Access connector resource.
---</rdfs:comment>
  </owl:Class>
  <owl:DatatypeProperty rdf:about="http://example.org/onto/prop/google_vpc_access_connector_connected_projects">
    <rdfs:label>connected_projects</rdfs:label>
    <rdfs:comment>List of projects using the connector.</rdfs:comment>
    <rdfs:domain rdf:resource="http://example.org/onto/class/google_vpc_access_connector"/>
    <rdfs:range rdf:resource="http://www.w3.org/2001/XMLSchema#string"/>
  </owl:DatatypeProperty>
  <owl:DatatypeProperty rdf:about="http://example.org/onto/prop/google_vpc_access_connector_id">
    <rdfs:label>id</rdfs:label>
    <rdfs:domain rdf:resource="http://example.org/onto/class/google_vpc_access_connector"/>
    <rdfs:range rdf:resource="http://www.w3.org/2001/XMLSchema#string"/>
  </owl:DatatypeProperty>
  <owl:DatatypeProperty rdf:about="http://example.org/onto/prop/google_vpc_access_connector_ip_cidr_range">
    <rdfs:label>ip_cidr_range</rdfs:label>
    <rdfs:comment>The range of internal addresses that follows RFC 4632 notation. Example: '10.132.0.0/28'.</rdfs:comment>
    <rdfs:domain rdf:resource="http://example.org/onto/class/google_vpc_access_connector"/>
    <rdfs:range rdf:resource="http://www.w3.org/2001/XMLSchema#string"/>
  </owl:DatatypeProperty>
  <owl:DatatypeProperty rdf:about="http://example.org/onto/prop/google_vpc_access_connector_machine_type">
    <rdfs:label>machine_type</rdfs:label>
    <rdfs:comment>Machine type of VM Instance underlying connector. Default is e2-micro</rdfs:comment>
    <rdfs:domain rdf:resource="http://example.org/onto/class/google_vpc_access_connector"/>
    <rdfs:range rdf:resource="http://www.w3.org/2001/XMLSchema#string"/>
  </owl:DatatypeProperty>
  <owl:DatatypeProperty rdf:about="http://example.org/onto/prop/google_vpc_access_connector_max_instances">
    <rdfs:label>max_instances</rdfs:label>
    <rdfs:comment>Maximum value of instances in autoscaling group underlying the connector. Value must be between 3 and 10, inclusive. Must be
higher than the value specified by min_instances. Required alongside 'min_instances' if not using 'min_throughput'/'max_throughput'.</rdfs:comment>
    <rdfs:domain rdf:resource="http://example.org/onto/class/google_vpc_access_connector"/>
    <rdfs:range rdf:resource="http://www.w3.org/2001/XMLSchema#string"/>
  </owl:DatatypeProperty>
  <owl:DatatypeProperty rdf:about="http://example.org/onto/prop/google_vpc_access_connector_max_throughput">
    <rdfs:label>max_throughput</rdfs:label>
    <rdfs:comment>Maximum throughput of the connector in Mbps, must be greater than 'min_throughput'. Default is 300. Refers to the expected throughput
when using an e2-micro machine type. Value must be a multiple of 100 from 300 through 1000. Must be higher than the value specified by
min_throughput. Only one of 'max_throughput' and 'max_instances' can be specified. The use of max_throughput is discouraged in favor of max_instances.</rdfs:comment>
    <rdfs:domain rdf:resource="http://example.org/onto/class/google_vpc_access_connector"/>
    <rdfs:range rdf:resource="http://www.w3.org/2001/XMLSchema#string"/>
  </owl:DatatypeProperty>
  <owl:DatatypeProperty rdf:about="http://example.org/onto/prop/google_vpc_access_connector_min_instances">
    <rdfs:label>min_instances</rdfs:label>
    <rdfs:comment>Minimum value of instances in autoscaling group underlying the connector. Value must be between 2 and 9, inclusive. Must be
lower than the value specified by max_instances. Required alongside 'max_instances' if not using 'min_throughput'/'max_throughput'.</rdfs:comment>
    <rdfs:domain rdf:resource="http://example.org/onto/class/google_vpc_access_connector"/>
    <rdfs:range rdf:resource="http://www.w3.org/2001/XMLSchema#string"/>
  </owl:DatatypeProperty>
  <owl:DatatypeProperty rdf:about="http://example.org/onto/prop/google_vpc_access_connector_min_throughput">
    <rdfs:label>min_throughput</rdfs:label>
    <rdfs:comment>Minimum throughput of the connector in Mbps. Default and min is 200. Refers to the expected throughput when using an e2-micro machine type.
Value must be a multiple of 100 from 200 through 900. Must be lower than the value specified by max_throughput.
Only one of 'min_throughput' and 'min_instances' can be specified. The use of min_throughput is discouraged in favor of min_instances.</rdfs:comment>
    <rdfs:domain rdf:resource="http://example.org/onto/class/google_vpc_access_connector"/>
    <rdfs:range rdf:resource="http://www.w3.org/2001/XMLSchema#string"/>
  </owl:DatatypeProperty>
  <owl:DatatypeProperty rdf:about="http://example.org/onto/prop/google_vpc_access_connector_name">
    <rdfs:label>name</rdfs:label>
    <rdfs:comment>The name of the resource (Max 25 characters).</rdfs:comment>
    <rdfs:domain rdf:resource="http://example.org/onto/class/google_vpc_access_connector"/>
    <rdfs:range rdf:resource="http://www.w3.org/2001/XMLSchema#string"/>
  </owl:DatatypeProperty>
  <owl:DatatypeProperty rdf:about="http://example.org/onto/prop/google_vpc_access_connector_network">
    <rdfs:label>network</rdfs:label>
    <rdfs:comment>Name or self_link of the VPC network. Required if 'ip_cidr_range' is set.</rdfs:comment>
    <rdfs:domain rdf:resource="http://example.org/onto/class/google_vpc_access_connector"/>
    <rdfs:range rdf:resource="http://www.w3.org/2001/XMLSchema#string"/>
  </owl:DatatypeProperty>
  <owl:DatatypeProperty rdf:about="http://example.org/onto/prop/google_vpc_access_connector_project">
    <rdfs:label>project</rdfs:label>
    <rdfs:domain rdf:resource="http://example.org/onto/class/google_vpc_access_connector"/>
    <rdfs:range rdf:resource="http://www.w3.org/2001/XMLSchema#string"/>
  </owl:DatatypeProperty>
  <owl:DatatypeProperty rdf:about="http://example.org/onto/prop/google_vpc_access_connector_region">
    <rdfs:label>region</rdfs:label>
    <rdfs:comment>Region where the VPC Access connector resides. If it is not provided, the provider region is used.</rdfs:comment>
    <rdfs:domain rdf:resource="http://example.org/onto/class/google_vpc_access_connector"/>
    <rdfs:range rdf:resource="http://www.w3.org/2001/XMLSchema#string"/>
  </owl:DatatypeProperty>
  <owl:DatatypeProperty rdf:about="http://example.org/onto/prop/google_vpc_access_connector_self_link">
    <rdfs:label>self_link</rdfs:label>
    <rdfs:comment>The fully qualified name of this VPC connector</rdfs:comment>
    <rdfs:domain rdf:resource="http://example.org/onto/class/google_vpc_access_connector"/>
    <rdfs:range rdf:resource="http://www.w3.org/2001/XMLSchema#string"/>
  </owl:DatatypeProperty>
  <owl:DatatypeProperty rdf:about="http://example.org/onto/prop/google_vpc_access_connector_state">
    <rdfs:label>state</rdfs:label>
    <rdfs:comment>State of the VPC access connector.</rdfs:comment>
    <rdfs:domain rdf:resource="http://example.org/onto/class/google_vpc_access_connector"/>
    <rdfs:range rdf:resource="http://www.w3.org/2001/XMLSchema#string"/>
  </owl:DatatypeProperty>
  <owl:DatatypeProperty rdf:about="http://example.org/onto/prop/google_vpc_access_connector_name">
    <rdfs:label>name</rdfs:label>
    <rdfs:comment>Subnet name (relative, not fully qualified). E.g. if the full subnet selfLink is
https://compute.googleapis.com/compute/v1/projects/{project}/regions/{region}/subnetworks/{subnetName} the correct input for this field would be {subnetName}"</rdfs:comment>
    <rdfs:domain rdf:resource="http://example.org/onto/class/google_vpc_access_connector"/>
    <rdfs:range rdf:resource="http://www.w3.org/2001/XMLSchema#string"/>
  </owl:DatatypeProperty>
  <owl:DatatypeProperty rdf:about="http://example.org/onto/prop/google_vpc_access_connector_project_id">
    <rdfs:label>project_id</rdfs:label>
    <rdfs:comment>Project in which the subnet exists. If not set, this project is assumed to be the project for which the connector create request was issued.</rdfs:comment>
    <rdfs:domain rdf:resource="http://example.org/onto/class/google_vpc_access_connector"/>
    <rdfs:range rdf:resource="http://www.w3.org/2001/XMLSchema#string"/>
  </owl:DatatypeProperty>
  <owl:DatatypeProperty rdf:about="http://example.org/onto/prop/google_vpc_access_connector_create">
    <rdfs:label>create</rdfs:label>
    <rdfs:domain rdf:resource="http://example.org/onto/class/google_vpc_access_connector"/>
    <rdfs:range rdf:resource="http://www.w3.org/2001/XMLSchema#string"/>
  </owl:DatatypeProperty>
  <owl:DatatypeProperty rdf:about="http://example.org/onto/prop/google_vpc_access_connector_delete">
    <rdfs:label>delete</rdfs:label>
    <rdfs:domain rdf:resource="http://example.org/onto/class/google_vpc_access_connector"/>
    <rdfs:range rdf:resource="http://www.w3.org/2001/XMLSchema#string"/>
  </owl:DatatypeProperty>
  <owl:DatatypeProperty rdf:about="http://example.org/onto/prop/google_vpc_access_connector_update">
    <rdfs:label>update</rdfs:label>
    <rdfs:domain rdf:resource="http://example.org/onto/class/google_vpc_access_connector"/>
    <rdfs:range rdf:resource="http://www.w3.org/2001/XMLSchema#string"/>
  </owl:DatatypeProperty>
</rdf:RDF>
