<?xml version="1.0" encoding="UTF-8"?>
<rdf:RDF
  xmlns:rdf="http://www.w3.org/1999/02/22-rdf-syntax-ns#"
  xmlns:rdfs="http://www.w3.org/2000/01/rdf-schema#"
  xmlns:owl="http://www.w3.org/2002/07/owl#"
  xmlns:xsd="http://www.w3.org/2001/XMLSchema#"
  xml:base="http://example.org/onto/">
  <owl:Class rdf:about="http://example.org/onto/class/google_logging_organization_settings">
    <rdfs:label>google_logging_organization_settings</rdfs:label>
    <rdfs:comment>#
#     ***     AUTO GENERATED CODE    ***    Type: MMv1     ***
#
# ----------------------------------------------------------------------------
#
#     This code is generated by Magic Modules using the following:
#
#     Configuration: https:#github.com/GoogleCloudPlatform/magic-modules/tree/main/mmv1/products/logging/OrganizationSettings.yaml
#     Template:      https:#github.com/GoogleCloudPlatform/magic-modules/tree/main/mmv1/templates/terraform/resource.html.markdown.tmpl
#
#     DO NOT EDIT this file directly. Any changes made to this file will be
#     overwritten during the next generation cycle.
#
# ----------------------------------------------------------------------------
subcategory: "Cloud (Stackdriver) Logging"
description: |-
  Default resource settings control whether CMEK is required for new log buckets.
---</rdfs:comment>
  </owl:Class>
  <owl:DatatypeProperty rdf:about="http://example.org/onto/prop/google_logging_organization_settings_disable_default_sink">
    <rdfs:label>disable_default_sink</rdfs:label>
    <rdfs:comment>If set to true, the _Default sink in newly created projects and folders will created in a disabled state. This can be used to automatically disable log storage if there is already an aggregated sink configured in the hierarchy. The _Default sink can be re-enabled manually if needed.</rdfs:comment>
    <rdfs:domain rdf:resource="http://example.org/onto/class/google_logging_organization_settings"/>
    <rdfs:range rdf:resource="http://www.w3.org/2001/XMLSchema#string"/>
  </owl:DatatypeProperty>
  <owl:DatatypeProperty rdf:about="http://example.org/onto/prop/google_logging_organization_settings_id">
    <rdfs:label>id</rdfs:label>
    <rdfs:domain rdf:resource="http://example.org/onto/class/google_logging_organization_settings"/>
    <rdfs:range rdf:resource="http://www.w3.org/2001/XMLSchema#string"/>
  </owl:DatatypeProperty>
  <owl:DatatypeProperty rdf:about="http://example.org/onto/prop/google_logging_organization_settings_kms_key_name">
    <rdfs:label>kms_key_name</rdfs:label>
    <rdfs:comment>The resource name for the configured Cloud KMS key.</rdfs:comment>
    <rdfs:domain rdf:resource="http://example.org/onto/class/google_logging_organization_settings"/>
    <rdfs:range rdf:resource="http://www.w3.org/2001/XMLSchema#string"/>
  </owl:DatatypeProperty>
  <owl:DatatypeProperty rdf:about="http://example.org/onto/prop/google_logging_organization_settings_kms_service_account_id">
    <rdfs:label>kms_service_account_id</rdfs:label>
    <rdfs:comment>The service account that will be used by the Log Router to access your Cloud KMS key.</rdfs:comment>
    <rdfs:domain rdf:resource="http://example.org/onto/class/google_logging_organization_settings"/>
    <rdfs:range rdf:resource="http://www.w3.org/2001/XMLSchema#string"/>
  </owl:DatatypeProperty>
  <owl:DatatypeProperty rdf:about="http://example.org/onto/prop/google_logging_organization_settings_logging_service_account_id">
    <rdfs:label>logging_service_account_id</rdfs:label>
    <rdfs:comment>The service account for the given container. Sinks use this service account as their writerIdentity if no custom service account is provided.</rdfs:comment>
    <rdfs:domain rdf:resource="http://example.org/onto/class/google_logging_organization_settings"/>
    <rdfs:range rdf:resource="http://www.w3.org/2001/XMLSchema#string"/>
  </owl:DatatypeProperty>
  <owl:DatatypeProperty rdf:about="http://example.org/onto/prop/google_logging_organization_settings_name">
    <rdfs:label>name</rdfs:label>
    <rdfs:comment>The resource name of the settings.</rdfs:comment>
    <rdfs:domain rdf:resource="http://example.org/onto/class/google_logging_organization_settings"/>
    <rdfs:range rdf:resource="http://www.w3.org/2001/XMLSchema#string"/>
  </owl:DatatypeProperty>
  <owl:DatatypeProperty rdf:about="http://example.org/onto/prop/google_logging_organization_settings_organization">
    <rdfs:label>organization</rdfs:label>
    <rdfs:comment>The organization for which to retrieve or configure settings.</rdfs:comment>
    <rdfs:domain rdf:resource="http://example.org/onto/class/google_logging_organization_settings"/>
    <rdfs:range rdf:resource="http://www.w3.org/2001/XMLSchema#string"/>
  </owl:DatatypeProperty>
  <owl:DatatypeProperty rdf:about="http://example.org/onto/prop/google_logging_organization_settings_storage_location">
    <rdfs:label>storage_location</rdfs:label>
    <rdfs:comment>The storage location that Cloud Logging will use to create new resources when a location is needed but not explicitly provided.</rdfs:comment>
    <rdfs:domain rdf:resource="http://example.org/onto/class/google_logging_organization_settings"/>
    <rdfs:range rdf:resource="http://www.w3.org/2001/XMLSchema#string"/>
  </owl:DatatypeProperty>
  <owl:DatatypeProperty rdf:about="http://example.org/onto/prop/google_logging_organization_settings_create">
    <rdfs:label>create</rdfs:label>
    <rdfs:domain rdf:resource="http://example.org/onto/class/google_logging_organization_settings"/>
    <rdfs:range rdf:resource="http://www.w3.org/2001/XMLSchema#string"/>
  </owl:DatatypeProperty>
  <owl:DatatypeProperty rdf:about="http://example.org/onto/prop/google_logging_organization_settings_delete">
    <rdfs:label>delete</rdfs:label>
    <rdfs:domain rdf:resource="http://example.org/onto/class/google_logging_organization_settings"/>
    <rdfs:range rdf:resource="http://www.w3.org/2001/XMLSchema#string"/>
  </owl:DatatypeProperty>
  <owl:DatatypeProperty rdf:about="http://example.org/onto/prop/google_logging_organization_settings_update">
    <rdfs:label>update</rdfs:label>
    <rdfs:domain rdf:resource="http://example.org/onto/class/google_logging_organization_settings"/>
    <rdfs:range rdf:resource="http://www.w3.org/2001/XMLSchema#string"/>
  </owl:DatatypeProperty>
</rdf:RDF>
