<?xml version="1.0" encoding="UTF-8"?>
<rdf:RDF
  xmlns:rdf="http://www.w3.org/1999/02/22-rdf-syntax-ns#"
  xmlns:rdfs="http://www.w3.org/2000/01/rdf-schema#"
  xmlns:owl="http://www.w3.org/2002/07/owl#"
  xmlns:xsd="http://www.w3.org/2001/XMLSchema#"
  xml:base="http://example.org/onto/">
  <owl:Class rdf:about="http://example.org/onto/class/google_compute_interconnect">
    <rdfs:label>google_compute_interconnect</rdfs:label>
    <rdfs:comment>#
#     ***     AUTO GENERATED CODE    ***    Type: MMv1     ***
#
# ----------------------------------------------------------------------------
#
#     This code is generated by Magic Modules using the following:
#
#     Configuration: https:#github.com/GoogleCloudPlatform/magic-modules/tree/main/mmv1/products/compute/Interconnect.yaml
#     Template:      https:#github.com/GoogleCloudPlatform/magic-modules/tree/main/mmv1/templates/terraform/resource.html.markdown.tmpl
#
#     DO NOT EDIT this file directly. Any changes made to this file will be
#     overwritten during the next generation cycle.
#
# ----------------------------------------------------------------------------
subcategory: "Compute Engine"
description: |-
  Represents an Interconnect resource.
---</rdfs:comment>
  </owl:Class>
  <owl:DatatypeProperty rdf:about="http://example.org/onto/prop/google_compute_interconnect_admin_enabled">
    <rdfs:label>admin_enabled</rdfs:label>
    <rdfs:comment>Administrative status of the interconnect. When this is set to true, the Interconnect is
functional and can carry traffic. When set to false, no packets can be carried over the
interconnect and no BGP routes are exchanged over it. By default, the status is set to true.</rdfs:comment>
    <rdfs:domain rdf:resource="http://example.org/onto/class/google_compute_interconnect"/>
    <rdfs:range rdf:resource="http://www.w3.org/2001/XMLSchema#string"/>
  </owl:DatatypeProperty>
  <owl:DatatypeProperty rdf:about="http://example.org/onto/prop/google_compute_interconnect_available_features">
    <rdfs:label>available_features</rdfs:label>
    <rdfs:comment>interconnects.list of features available for this Interconnect connection. Can take the value:
MACSEC. If present then the Interconnect connection is provisioned on MACsec capable hardware
ports. If not present then the Interconnect connection is provisioned on non-MACsec capable
ports and MACsec isn't supported and enabling MACsec fails).</rdfs:comment>
    <rdfs:domain rdf:resource="http://example.org/onto/class/google_compute_interconnect"/>
    <rdfs:range rdf:resource="http://www.w3.org/2001/XMLSchema#string"/>
  </owl:DatatypeProperty>
  <owl:DatatypeProperty rdf:about="http://example.org/onto/prop/google_compute_interconnect_circuit_infos">
    <rdfs:label>circuit_infos</rdfs:label>
    <rdfs:comment>A list of CircuitInfo objects, that describe the individual circuits in this LAG.</rdfs:comment>
    <rdfs:domain rdf:resource="http://example.org/onto/class/google_compute_interconnect"/>
    <rdfs:range rdf:resource="http://www.w3.org/2001/XMLSchema#string"/>
  </owl:DatatypeProperty>
  <owl:DatatypeProperty rdf:about="http://example.org/onto/prop/google_compute_interconnect_creation_timestamp">
    <rdfs:label>creation_timestamp</rdfs:label>
    <rdfs:comment>Creation timestamp in RFC3339 text format.</rdfs:comment>
    <rdfs:domain rdf:resource="http://example.org/onto/class/google_compute_interconnect"/>
    <rdfs:range rdf:resource="http://www.w3.org/2001/XMLSchema#string"/>
  </owl:DatatypeProperty>
  <owl:DatatypeProperty rdf:about="http://example.org/onto/prop/google_compute_interconnect_customer_name">
    <rdfs:label>customer_name</rdfs:label>
    <rdfs:comment>Customer name, to put in the Letter of Authorization as the party authorized to request a
crossconnect. This field is required for Dedicated and Partner Interconnect, should not be specified
for cross-cloud interconnect.</rdfs:comment>
    <rdfs:domain rdf:resource="http://example.org/onto/class/google_compute_interconnect"/>
    <rdfs:range rdf:resource="http://www.w3.org/2001/XMLSchema#string"/>
  </owl:DatatypeProperty>
  <owl:DatatypeProperty rdf:about="http://example.org/onto/prop/google_compute_interconnect_description">
    <rdfs:label>description</rdfs:label>
    <rdfs:comment>An optional description of this resource. Provide this property when you create the resource.</rdfs:comment>
    <rdfs:domain rdf:resource="http://example.org/onto/class/google_compute_interconnect"/>
    <rdfs:range rdf:resource="http://www.w3.org/2001/XMLSchema#string"/>
  </owl:DatatypeProperty>
  <owl:DatatypeProperty rdf:about="http://example.org/onto/prop/google_compute_interconnect_effective_labels">
    <rdfs:label>effective_labels</rdfs:label>
    <rdfs:comment>All of labels (key/value pairs) present on the resource in GCP, including the labels configured through Terraform, other clients and services.</rdfs:comment>
    <rdfs:domain rdf:resource="http://example.org/onto/class/google_compute_interconnect"/>
    <rdfs:range rdf:resource="http://www.w3.org/2001/XMLSchema#string"/>
  </owl:DatatypeProperty>
  <owl:DatatypeProperty rdf:about="http://example.org/onto/prop/google_compute_interconnect_expected_outages">
    <rdfs:label>expected_outages</rdfs:label>
    <rdfs:comment>A list of outages expected for this Interconnect.</rdfs:comment>
    <rdfs:domain rdf:resource="http://example.org/onto/class/google_compute_interconnect"/>
    <rdfs:range rdf:resource="http://www.w3.org/2001/XMLSchema#string"/>
  </owl:DatatypeProperty>
  <owl:DatatypeProperty rdf:about="http://example.org/onto/prop/google_compute_interconnect_google_ip_address">
    <rdfs:label>google_ip_address</rdfs:label>
    <rdfs:comment>IP address configured on the Google side of the Interconnect link.
This can be used only for ping tests.</rdfs:comment>
    <rdfs:domain rdf:resource="http://example.org/onto/class/google_compute_interconnect"/>
    <rdfs:range rdf:resource="http://www.w3.org/2001/XMLSchema#string"/>
  </owl:DatatypeProperty>
  <owl:DatatypeProperty rdf:about="http://example.org/onto/prop/google_compute_interconnect_google_reference_id">
    <rdfs:label>google_reference_id</rdfs:label>
    <rdfs:comment>Google reference ID to be used when raising support tickets with Google or otherwise to debug
backend connectivity issues.</rdfs:comment>
    <rdfs:domain rdf:resource="http://example.org/onto/class/google_compute_interconnect"/>
    <rdfs:range rdf:resource="http://www.w3.org/2001/XMLSchema#string"/>
  </owl:DatatypeProperty>
  <owl:DatatypeProperty rdf:about="http://example.org/onto/prop/google_compute_interconnect_id">
    <rdfs:label>id</rdfs:label>
    <rdfs:domain rdf:resource="http://example.org/onto/class/google_compute_interconnect"/>
    <rdfs:range rdf:resource="http://www.w3.org/2001/XMLSchema#string"/>
  </owl:DatatypeProperty>
  <owl:DatatypeProperty rdf:about="http://example.org/onto/prop/google_compute_interconnect_interconnect_attachments">
    <rdfs:label>interconnect_attachments</rdfs:label>
    <rdfs:comment>A list of the URLs of all InterconnectAttachments configured to use this Interconnect.</rdfs:comment>
    <rdfs:domain rdf:resource="http://example.org/onto/class/google_compute_interconnect"/>
    <rdfs:range rdf:resource="http://www.w3.org/2001/XMLSchema#string"/>
  </owl:DatatypeProperty>
  <owl:DatatypeProperty rdf:about="http://example.org/onto/prop/google_compute_interconnect_interconnect_groups">
    <rdfs:label>interconnect_groups</rdfs:label>
    <rdfs:comment>URLs of InterconnectGroups that include this Interconnect.
Order is arbitrary and items are unique.</rdfs:comment>
    <rdfs:domain rdf:resource="http://example.org/onto/class/google_compute_interconnect"/>
    <rdfs:range rdf:resource="http://www.w3.org/2001/XMLSchema#string"/>
  </owl:DatatypeProperty>
  <owl:DatatypeProperty rdf:about="http://example.org/onto/prop/google_compute_interconnect_interconnect_type">
    <rdfs:label>interconnect_type</rdfs:label>
    <rdfs:comment>Type of interconnect. Note that a value IT_PRIVATE has been deprecated in favor of DEDICATED.
Can take one of the following values:
  - PARTNER: A partner-managed interconnection shared between customers though a partner.
  - DEDICATED: A dedicated physical interconnection with the customer. Possible values: ["DEDICATED", "PARTNER", "IT_PRIVATE"]</rdfs:comment>
    <rdfs:domain rdf:resource="http://example.org/onto/class/google_compute_interconnect"/>
    <rdfs:range rdf:resource="http://www.w3.org/2001/XMLSchema#string"/>
  </owl:DatatypeProperty>
  <owl:DatatypeProperty rdf:about="http://example.org/onto/prop/google_compute_interconnect_label_fingerprint">
    <rdfs:label>label_fingerprint</rdfs:label>
    <rdfs:comment>A fingerprint for the labels being applied to this Interconnect, which is essentially a hash
of the labels set used for optimistic locking. The fingerprint is initially generated by
Compute Engine and changes after every request to modify or update labels.
You must always provide an up-to-date fingerprint hash in order to update or change labels,
otherwise the request will fail with error 412 conditionNotMet.</rdfs:comment>
    <rdfs:domain rdf:resource="http://example.org/onto/class/google_compute_interconnect"/>
    <rdfs:range rdf:resource="http://www.w3.org/2001/XMLSchema#string"/>
  </owl:DatatypeProperty>
  <owl:DatatypeProperty rdf:about="http://example.org/onto/prop/google_compute_interconnect_labels">
    <rdfs:label>labels</rdfs:label>
    <rdfs:comment>Labels for this resource. These can only be added or modified by the setLabels
method. Each label key/value pair must comply with RFC1035. Label values may be empty.


**Note**: This field is non-authoritative, and will only manage the labels present in your configuration.
Please refer to the field 'effective_labels' for all of the labels present on the resource.</rdfs:comment>
    <rdfs:domain rdf:resource="http://example.org/onto/class/google_compute_interconnect"/>
    <rdfs:range rdf:resource="http://www.w3.org/2001/XMLSchema#string"/>
  </owl:DatatypeProperty>
  <owl:DatatypeProperty rdf:about="http://example.org/onto/prop/google_compute_interconnect_link_type">
    <rdfs:label>link_type</rdfs:label>
    <rdfs:comment>Type of link requested. Note that this field indicates the speed of each of the links in the
bundle, not the speed of the entire bundle. Can take one of the following values:
  - LINK_TYPE_ETHERNET_10G_LR: A 10G Ethernet with LR optics.
  - LINK_TYPE_ETHERNET_100G_LR: A 100G Ethernet with LR optics.
  - LINK_TYPE_ETHERNET_400G_LR4: A 400G Ethernet with LR4 optics Possible values: ["LINK_TYPE_ETHERNET_10G_LR", "LINK_TYPE_ETHERNET_100G_LR", "LINK_TYPE_ETHERNET_400G_LR4"]</rdfs:comment>
    <rdfs:domain rdf:resource="http://example.org/onto/class/google_compute_interconnect"/>
    <rdfs:range rdf:resource="http://www.w3.org/2001/XMLSchema#string"/>
  </owl:DatatypeProperty>
  <owl:DatatypeProperty rdf:about="http://example.org/onto/prop/google_compute_interconnect_location">
    <rdfs:label>location</rdfs:label>
    <rdfs:comment>URL of the InterconnectLocation object that represents where this connection is to be provisioned.
Specifies the location inside Google's Networks.</rdfs:comment>
    <rdfs:domain rdf:resource="http://example.org/onto/class/google_compute_interconnect"/>
    <rdfs:range rdf:resource="http://www.w3.org/2001/XMLSchema#string"/>
  </owl:DatatypeProperty>
  <owl:DatatypeProperty rdf:about="http://example.org/onto/prop/google_compute_interconnect_macsec_enabled">
    <rdfs:label>macsec_enabled</rdfs:label>
    <rdfs:comment>Enable or disable MACsec on this Interconnect connection.
MACsec enablement fails if the MACsec object is not specified.</rdfs:comment>
    <rdfs:domain rdf:resource="http://example.org/onto/class/google_compute_interconnect"/>
    <rdfs:range rdf:resource="http://www.w3.org/2001/XMLSchema#string"/>
  </owl:DatatypeProperty>
  <owl:DatatypeProperty rdf:about="http://example.org/onto/prop/google_compute_interconnect_name">
    <rdfs:label>name</rdfs:label>
    <rdfs:comment>Name of the resource. Provided by the client when the resource is created. The name must be
1-63 characters long, and comply with RFC1035. Specifically, the name must be 1-63 characters
long and match the regular expression '[a-z]([-a-z0-9]*[a-z0-9])?' which means the first
character must be a lowercase letter, and all following characters must be a dash,
lowercase letter, or digit, except the last character, which cannot be a dash.</rdfs:comment>
    <rdfs:domain rdf:resource="http://example.org/onto/class/google_compute_interconnect"/>
    <rdfs:range rdf:resource="http://www.w3.org/2001/XMLSchema#string"/>
  </owl:DatatypeProperty>
  <owl:DatatypeProperty rdf:about="http://example.org/onto/prop/google_compute_interconnect_noc_contact_email">
    <rdfs:label>noc_contact_email</rdfs:label>
    <rdfs:comment>Email address to contact the customer NOC for operations and maintenance notifications
regarding this Interconnect. If specified, this will be used for notifications in addition to
all other forms described, such as Cloud Monitoring logs alerting and Cloud Notifications.
This field is required for users who sign up for Cloud Interconnect using workforce identity
federation.</rdfs:comment>
    <rdfs:domain rdf:resource="http://example.org/onto/class/google_compute_interconnect"/>
    <rdfs:range rdf:resource="http://www.w3.org/2001/XMLSchema#string"/>
  </owl:DatatypeProperty>
  <owl:DatatypeProperty rdf:about="http://example.org/onto/prop/google_compute_interconnect_operational_status">
    <rdfs:label>operational_status</rdfs:label>
    <rdfs:comment>The current status of this Interconnect's functionality, which can take one of the following:
  - OS_ACTIVE: A valid Interconnect, which is turned up and is ready to use. Attachments may
  be provisioned on this Interconnect.
  - OS_UNPROVISIONED: An Interconnect that has not completed turnup. No attachments may be
  provisioned on this Interconnect.
  - OS_UNDER_MAINTENANCE: An Interconnect that is undergoing internal maintenance. No
  attachments may be provisioned or updated on this Interconnect.</rdfs:comment>
    <rdfs:domain rdf:resource="http://example.org/onto/class/google_compute_interconnect"/>
    <rdfs:range rdf:resource="http://www.w3.org/2001/XMLSchema#string"/>
  </owl:DatatypeProperty>
  <owl:DatatypeProperty rdf:about="http://example.org/onto/prop/google_compute_interconnect_peer_ip_address">
    <rdfs:label>peer_ip_address</rdfs:label>
    <rdfs:comment>IP address configured on the customer side of the Interconnect link.
The customer should configure this IP address during turnup when prompted by Google NOC.
This can be used only for ping tests.</rdfs:comment>
    <rdfs:domain rdf:resource="http://example.org/onto/class/google_compute_interconnect"/>
    <rdfs:range rdf:resource="http://www.w3.org/2001/XMLSchema#string"/>
  </owl:DatatypeProperty>
  <owl:DatatypeProperty rdf:about="http://example.org/onto/prop/google_compute_interconnect_project">
    <rdfs:label>project</rdfs:label>
    <rdfs:domain rdf:resource="http://example.org/onto/class/google_compute_interconnect"/>
    <rdfs:range rdf:resource="http://www.w3.org/2001/XMLSchema#string"/>
  </owl:DatatypeProperty>
  <owl:DatatypeProperty rdf:about="http://example.org/onto/prop/google_compute_interconnect_provisioned_link_count">
    <rdfs:label>provisioned_link_count</rdfs:label>
    <rdfs:comment>Number of links actually provisioned in this interconnect.</rdfs:comment>
    <rdfs:domain rdf:resource="http://example.org/onto/class/google_compute_interconnect"/>
    <rdfs:range rdf:resource="http://www.w3.org/2001/XMLSchema#string"/>
  </owl:DatatypeProperty>
  <owl:DatatypeProperty rdf:about="http://example.org/onto/prop/google_compute_interconnect_remote_location">
    <rdfs:label>remote_location</rdfs:label>
    <rdfs:comment>Indicates that this is a Cross-Cloud Interconnect. This field specifies the location outside
of Google's network that the interconnect is connected to.</rdfs:comment>
    <rdfs:domain rdf:resource="http://example.org/onto/class/google_compute_interconnect"/>
    <rdfs:range rdf:resource="http://www.w3.org/2001/XMLSchema#string"/>
  </owl:DatatypeProperty>
  <owl:DatatypeProperty rdf:about="http://example.org/onto/prop/google_compute_interconnect_requested_features">
    <rdfs:label>requested_features</rdfs:label>
    <rdfs:comment>interconnects.list of features requested for this Interconnect connection. Options: IF_MACSEC (
If specified then the connection is created on MACsec capable hardware ports. If not
specified, the default value is false, which allocates non-MACsec capable ports first if
available). Note that MACSEC is still technically allowed for compatibility reasons, but it
does not work with the API, and will be removed in an upcoming major version. Possible values: ["MACSEC", "CROSS_SITE_NETWORK", "IF_MACSEC"]</rdfs:comment>
    <rdfs:domain rdf:resource="http://example.org/onto/class/google_compute_interconnect"/>
    <rdfs:range rdf:resource="http://www.w3.org/2001/XMLSchema#string"/>
  </owl:DatatypeProperty>
  <owl:DatatypeProperty rdf:about="http://example.org/onto/prop/google_compute_interconnect_requested_link_count">
    <rdfs:label>requested_link_count</rdfs:label>
    <rdfs:comment>Target number of physical links in the link bundle, as requested by the customer.</rdfs:comment>
    <rdfs:domain rdf:resource="http://example.org/onto/class/google_compute_interconnect"/>
    <rdfs:range rdf:resource="http://www.w3.org/2001/XMLSchema#string"/>
  </owl:DatatypeProperty>
  <owl:DatatypeProperty rdf:about="http://example.org/onto/prop/google_compute_interconnect_satisfies_pzs">
    <rdfs:label>satisfies_pzs</rdfs:label>
    <rdfs:comment>Reserved for future use.</rdfs:comment>
    <rdfs:domain rdf:resource="http://example.org/onto/class/google_compute_interconnect"/>
    <rdfs:range rdf:resource="http://www.w3.org/2001/XMLSchema#string"/>
  </owl:DatatypeProperty>
  <owl:DatatypeProperty rdf:about="http://example.org/onto/prop/google_compute_interconnect_state">
    <rdfs:label>state</rdfs:label>
    <rdfs:comment>The current state of Interconnect functionality, which can take one of the following values:
  - ACTIVE: The Interconnect is valid, turned up and ready to use.
  Attachments may be provisioned on this Interconnect.
  - UNPROVISIONED: The Interconnect has not completed turnup. No attachments may b
   provisioned on this Interconnect.
  - UNDER_MAINTENANCE: The Interconnect is undergoing internal maintenance. No attachments may
   be provisioned or updated on this Interconnect.</rdfs:comment>
    <rdfs:domain rdf:resource="http://example.org/onto/class/google_compute_interconnect"/>
    <rdfs:range rdf:resource="http://www.w3.org/2001/XMLSchema#string"/>
  </owl:DatatypeProperty>
  <owl:DatatypeProperty rdf:about="http://example.org/onto/prop/google_compute_interconnect_terraform_labels">
    <rdfs:label>terraform_labels</rdfs:label>
    <rdfs:comment>The combination of labels configured directly on the resource
 and default labels configured on the provider.</rdfs:comment>
    <rdfs:domain rdf:resource="http://example.org/onto/class/google_compute_interconnect"/>
    <rdfs:range rdf:resource="http://www.w3.org/2001/XMLSchema#string"/>
  </owl:DatatypeProperty>
  <owl:DatatypeProperty rdf:about="http://example.org/onto/prop/google_compute_interconnect_fail_open">
    <rdfs:label>fail_open</rdfs:label>
    <rdfs:comment>If set to true, the Interconnect connection is configured with a should-secure
MACsec security policy, that allows the Google router to fallback to cleartext
traffic if the MKA session cannot be established. By default, the Interconnect
connection is configured with a must-secure security policy that drops all traffic
if the MKA session cannot be established with your router.</rdfs:comment>
    <rdfs:domain rdf:resource="http://example.org/onto/class/google_compute_interconnect"/>
    <rdfs:range rdf:resource="http://www.w3.org/2001/XMLSchema#string"/>
  </owl:DatatypeProperty>
  <owl:DatatypeProperty rdf:about="http://example.org/onto/prop/google_compute_interconnect_fail_open">
    <rdfs:label>fail_open</rdfs:label>
    <rdfs:comment>If set to true, the Interconnect connection is configured with a should-secure
MACsec security policy, that allows the Google router to fallback to cleartext
traffic if the MKA session cannot be established. By default, the Interconnect
connection is configured with a must-secure security policy that drops all traffic
if the MKA session cannot be established with your router.</rdfs:comment>
    <rdfs:domain rdf:resource="http://example.org/onto/class/google_compute_interconnect"/>
    <rdfs:range rdf:resource="http://www.w3.org/2001/XMLSchema#string"/>
  </owl:DatatypeProperty>
  <owl:DatatypeProperty rdf:about="http://example.org/onto/prop/google_compute_interconnect_name">
    <rdfs:label>name</rdfs:label>
    <rdfs:comment>A name for this pre-shared key. The name must be 1-63 characters long, and
 comply with RFC1035. Specifically, the name must be 1-63 characters long and match
 the regular expression '[a-z]([-a-z0-9]*[a-z0-9])?' which means the first character
 must be a lowercase letter, and all following characters must be a dash, lowercase
 letter, or digit, except the last character, which cannot be a dash.</rdfs:comment>
    <rdfs:domain rdf:resource="http://example.org/onto/class/google_compute_interconnect"/>
    <rdfs:range rdf:resource="http://www.w3.org/2001/XMLSchema#string"/>
  </owl:DatatypeProperty>
  <owl:DatatypeProperty rdf:about="http://example.org/onto/prop/google_compute_interconnect_start_time">
    <rdfs:label>start_time</rdfs:label>
    <rdfs:comment>A RFC3339 timestamp on or after which the key is valid. startTime can be in the
future. If the keychain has a single key, startTime can be omitted. If the keychain
has multiple keys, startTime is mandatory for each key. The start times of keys must
be in increasing order. The start times of two consecutive keys must be at least 6
hours apart.</rdfs:comment>
    <rdfs:domain rdf:resource="http://example.org/onto/class/google_compute_interconnect"/>
    <rdfs:range rdf:resource="http://www.w3.org/2001/XMLSchema#string"/>
  </owl:DatatypeProperty>
  <owl:DatatypeProperty rdf:about="http://example.org/onto/prop/google_compute_interconnect_create">
    <rdfs:label>create</rdfs:label>
    <rdfs:domain rdf:resource="http://example.org/onto/class/google_compute_interconnect"/>
    <rdfs:range rdf:resource="http://www.w3.org/2001/XMLSchema#string"/>
  </owl:DatatypeProperty>
  <owl:DatatypeProperty rdf:about="http://example.org/onto/prop/google_compute_interconnect_delete">
    <rdfs:label>delete</rdfs:label>
    <rdfs:domain rdf:resource="http://example.org/onto/class/google_compute_interconnect"/>
    <rdfs:range rdf:resource="http://www.w3.org/2001/XMLSchema#string"/>
  </owl:DatatypeProperty>
  <owl:DatatypeProperty rdf:about="http://example.org/onto/prop/google_compute_interconnect_update">
    <rdfs:label>update</rdfs:label>
    <rdfs:domain rdf:resource="http://example.org/onto/class/google_compute_interconnect"/>
    <rdfs:range rdf:resource="http://www.w3.org/2001/XMLSchema#string"/>
  </owl:DatatypeProperty>
</rdf:RDF>
