<?xml version="1.0" encoding="UTF-8"?>
<rdf:RDF
  xmlns:rdf="http://www.w3.org/1999/02/22-rdf-syntax-ns#"
  xmlns:rdfs="http://www.w3.org/2000/01/rdf-schema#"
  xmlns:owl="http://www.w3.org/2002/07/owl#"
  xmlns:xsd="http://www.w3.org/2001/XMLSchema#"
  xml:base="http://example.org/onto/">
  <owl:Class rdf:about="http://example.org/onto/class/google_os_config_v2_policy_orchestrator_for_organization">
    <rdfs:label>google_os_config_v2_policy_orchestrator_for_organization</rdfs:label>
    <rdfs:comment>#
#     ***     AUTO GENERATED CODE    ***    Type: MMv1     ***
#
# ----------------------------------------------------------------------------
#
#     This code is generated by Magic Modules using the following:
#
#     Configuration: https:#github.com/GoogleCloudPlatform/magic-modules/tree/main/mmv1/products/osconfigv2/PolicyOrchestratorForOrganization.yaml
#     Template:      https:#github.com/GoogleCloudPlatform/magic-modules/tree/main/mmv1/templates/terraform/resource.html.markdown.tmpl
#
#     DO NOT EDIT this file directly. Any changes made to this file will be
#     overwritten during the next generation cycle.
#
# ----------------------------------------------------------------------------
subcategory: "OS Config v2"
description: |-
  PolicyOrchestrator helps managing project+zone level policy resources (e.
---</rdfs:comment>
  </owl:Class>
  <owl:DatatypeProperty rdf:about="http://example.org/onto/prop/google_os_config_v2_policy_orchestrator_for_organization_action">
    <rdfs:label>action</rdfs:label>
    <rdfs:comment>Required. Action to be done by the orchestrator in
'projects/{project_id}/zones/{zone_id}' locations defined by the
'orchestration_scope'. Allowed values:
- 'UPSERT' - Orchestrator will create or update target resources.
- 'DELETE' - Orchestrator will delete target resources, if they exist</rdfs:comment>
    <rdfs:domain rdf:resource="http://example.org/onto/class/google_os_config_v2_policy_orchestrator_for_organization"/>
    <rdfs:range rdf:resource="http://www.w3.org/2001/XMLSchema#string"/>
  </owl:DatatypeProperty>
  <owl:DatatypeProperty rdf:about="http://example.org/onto/prop/google_os_config_v2_policy_orchestrator_for_organization_create_time">
    <rdfs:label>create_time</rdfs:label>
    <rdfs:comment>Output only. Timestamp when the policy orchestrator resource was created.</rdfs:comment>
    <rdfs:domain rdf:resource="http://example.org/onto/class/google_os_config_v2_policy_orchestrator_for_organization"/>
    <rdfs:range rdf:resource="http://www.w3.org/2001/XMLSchema#string"/>
  </owl:DatatypeProperty>
  <owl:DatatypeProperty rdf:about="http://example.org/onto/prop/google_os_config_v2_policy_orchestrator_for_organization_description">
    <rdfs:label>description</rdfs:label>
    <rdfs:comment>Optional. Freeform text describing the purpose of the resource.</rdfs:comment>
    <rdfs:domain rdf:resource="http://example.org/onto/class/google_os_config_v2_policy_orchestrator_for_organization"/>
    <rdfs:range rdf:resource="http://www.w3.org/2001/XMLSchema#string"/>
  </owl:DatatypeProperty>
  <owl:DatatypeProperty rdf:about="http://example.org/onto/prop/google_os_config_v2_policy_orchestrator_for_organization_effective_labels">
    <rdfs:label>effective_labels</rdfs:label>
    <rdfs:comment>All of labels (key/value pairs) present on the resource in GCP, including the labels configured through Terraform, other clients and services.</rdfs:comment>
    <rdfs:domain rdf:resource="http://example.org/onto/class/google_os_config_v2_policy_orchestrator_for_organization"/>
    <rdfs:range rdf:resource="http://www.w3.org/2001/XMLSchema#string"/>
  </owl:DatatypeProperty>
  <owl:DatatypeProperty rdf:about="http://example.org/onto/prop/google_os_config_v2_policy_orchestrator_for_organization_etag">
    <rdfs:label>etag</rdfs:label>
    <rdfs:comment>Output only. This checksum is computed by the server based on the value of other
fields, and may be sent on update and delete requests to ensure the
client has an up-to-date value before proceeding.</rdfs:comment>
    <rdfs:domain rdf:resource="http://example.org/onto/class/google_os_config_v2_policy_orchestrator_for_organization"/>
    <rdfs:range rdf:resource="http://www.w3.org/2001/XMLSchema#string"/>
  </owl:DatatypeProperty>
  <owl:DatatypeProperty rdf:about="http://example.org/onto/prop/google_os_config_v2_policy_orchestrator_for_organization_id">
    <rdfs:label>id</rdfs:label>
    <rdfs:domain rdf:resource="http://example.org/onto/class/google_os_config_v2_policy_orchestrator_for_organization"/>
    <rdfs:range rdf:resource="http://www.w3.org/2001/XMLSchema#string"/>
  </owl:DatatypeProperty>
  <owl:DatatypeProperty rdf:about="http://example.org/onto/prop/google_os_config_v2_policy_orchestrator_for_organization_labels">
    <rdfs:label>labels</rdfs:label>
    <rdfs:comment>Optional. Labels as key value pairs

**Note**: This field is non-authoritative, and will only manage the labels present in your configuration.
Please refer to the field 'effective_labels' for all of the labels present on the resource.</rdfs:comment>
    <rdfs:domain rdf:resource="http://example.org/onto/class/google_os_config_v2_policy_orchestrator_for_organization"/>
    <rdfs:range rdf:resource="http://www.w3.org/2001/XMLSchema#string"/>
  </owl:DatatypeProperty>
  <owl:DatatypeProperty rdf:about="http://example.org/onto/prop/google_os_config_v2_policy_orchestrator_for_organization_name">
    <rdfs:label>name</rdfs:label>
    <rdfs:comment>Immutable. Identifier. In form of
* 'organizations/{organization_id}/locations/global/policyOrchestrators/{orchestrator_id}'
* 'folders/{folder_id}/locations/global/policyOrchestrators/{orchestrator_id}'
* 'projects/{project_id_or_number}/locations/global/policyOrchestrators/{orchestrator_id}'</rdfs:comment>
    <rdfs:domain rdf:resource="http://example.org/onto/class/google_os_config_v2_policy_orchestrator_for_organization"/>
    <rdfs:range rdf:resource="http://www.w3.org/2001/XMLSchema#string"/>
  </owl:DatatypeProperty>
  <owl:DatatypeProperty rdf:about="http://example.org/onto/prop/google_os_config_v2_policy_orchestrator_for_organization_orchestration_state">
    <rdfs:label>orchestration_state</rdfs:label>
    <rdfs:comment>Describes the state of the orchestration process.</rdfs:comment>
    <rdfs:domain rdf:resource="http://example.org/onto/class/google_os_config_v2_policy_orchestrator_for_organization"/>
    <rdfs:range rdf:resource="http://www.w3.org/2001/XMLSchema#string"/>
  </owl:DatatypeProperty>
  <owl:DatatypeProperty rdf:about="http://example.org/onto/prop/google_os_config_v2_policy_orchestrator_for_organization_organization_id">
    <rdfs:label>organization_id</rdfs:label>
    <rdfs:comment>Part of 'parent'. Required. The parent resource name in the form of:
* 'organizations/{organization_id}/locations/global'
* 'folders/{folder_id}/locations/global'
* 'projects/{project_id_or_number}/locations/global'</rdfs:comment>
    <rdfs:domain rdf:resource="http://example.org/onto/class/google_os_config_v2_policy_orchestrator_for_organization"/>
    <rdfs:range rdf:resource="http://www.w3.org/2001/XMLSchema#string"/>
  </owl:DatatypeProperty>
  <owl:DatatypeProperty rdf:about="http://example.org/onto/prop/google_os_config_v2_policy_orchestrator_for_organization_policy_orchestrator_id">
    <rdfs:label>policy_orchestrator_id</rdfs:label>
    <rdfs:comment>Required. The logical identifier of the policy orchestrator, with the following
restrictions:

* Must contain only lowercase letters, numbers, and hyphens.
* Must start with a letter.
* Must be between 1-63 characters.
* Must end with a number or a letter.
* Must be unique within the parent.</rdfs:comment>
    <rdfs:domain rdf:resource="http://example.org/onto/class/google_os_config_v2_policy_orchestrator_for_organization"/>
    <rdfs:range rdf:resource="http://www.w3.org/2001/XMLSchema#string"/>
  </owl:DatatypeProperty>
  <owl:DatatypeProperty rdf:about="http://example.org/onto/prop/google_os_config_v2_policy_orchestrator_for_organization_reconciling">
    <rdfs:label>reconciling</rdfs:label>
    <rdfs:comment>Output only. Set to true, if the there are ongoing changes being applied by the
orchestrator.</rdfs:comment>
    <rdfs:domain rdf:resource="http://example.org/onto/class/google_os_config_v2_policy_orchestrator_for_organization"/>
    <rdfs:range rdf:resource="http://www.w3.org/2001/XMLSchema#string"/>
  </owl:DatatypeProperty>
  <owl:DatatypeProperty rdf:about="http://example.org/onto/prop/google_os_config_v2_policy_orchestrator_for_organization_state">
    <rdfs:label>state</rdfs:label>
    <rdfs:comment>Optional. State of the orchestrator. Can be updated to change orchestrator behaviour.
Allowed values:
- 'ACTIVE' - orchestrator is actively looking for actions to be taken.
- 'STOPPED' - orchestrator won't make any changes.

Note: There might be more states added in the future. We use string here
instead of an enum, to avoid the need of propagating new states to all the
client code.</rdfs:comment>
    <rdfs:domain rdf:resource="http://example.org/onto/class/google_os_config_v2_policy_orchestrator_for_organization"/>
    <rdfs:range rdf:resource="http://www.w3.org/2001/XMLSchema#string"/>
  </owl:DatatypeProperty>
  <owl:DatatypeProperty rdf:about="http://example.org/onto/prop/google_os_config_v2_policy_orchestrator_for_organization_terraform_labels">
    <rdfs:label>terraform_labels</rdfs:label>
    <rdfs:comment>The combination of labels configured directly on the resource
 and default labels configured on the provider.</rdfs:comment>
    <rdfs:domain rdf:resource="http://example.org/onto/class/google_os_config_v2_policy_orchestrator_for_organization"/>
    <rdfs:range rdf:resource="http://www.w3.org/2001/XMLSchema#string"/>
  </owl:DatatypeProperty>
  <owl:DatatypeProperty rdf:about="http://example.org/onto/prop/google_os_config_v2_policy_orchestrator_for_organization_update_time">
    <rdfs:label>update_time</rdfs:label>
    <rdfs:comment>Output only. Timestamp when the policy orchestrator resource was last modified.</rdfs:comment>
    <rdfs:domain rdf:resource="http://example.org/onto/class/google_os_config_v2_policy_orchestrator_for_organization"/>
    <rdfs:range rdf:resource="http://www.w3.org/2001/XMLSchema#string"/>
  </owl:DatatypeProperty>
  <owl:DatatypeProperty rdf:about="http://example.org/onto/prop/google_os_config_v2_policy_orchestrator_for_organization_id">
    <rdfs:label>id</rdfs:label>
    <rdfs:comment>Optional. ID of the resource to be used while generating set of affected resources.

For UPSERT action the value is auto-generated during PolicyOrchestrator
creation when not set. When the value is set it should following next
restrictions:

* Must contain only lowercase letters, numbers, and hyphens.
* Must start with a letter.
* Must be between 1-63 characters.
* Must end with a number or a letter.
* Must be unique within the project.

For DELETE action, ID must be specified explicitly during
PolicyOrchestrator creation.</rdfs:comment>
    <rdfs:domain rdf:resource="http://example.org/onto/class/google_os_config_v2_policy_orchestrator_for_organization"/>
    <rdfs:range rdf:resource="http://www.w3.org/2001/XMLSchema#string"/>
  </owl:DatatypeProperty>
  <owl:DatatypeProperty rdf:about="http://example.org/onto/prop/google_os_config_v2_policy_orchestrator_for_organization_baseline">
    <rdfs:label>baseline</rdfs:label>
    <rdfs:comment>Output only. Indicates that this revision has been successfully rolled out in this zone
and new VMs will be assigned OS policies from this revision.

For a given OS policy assignment, there is only one revision with a value
of 'true' for this field.</rdfs:comment>
    <rdfs:domain rdf:resource="http://example.org/onto/class/google_os_config_v2_policy_orchestrator_for_organization"/>
    <rdfs:range rdf:resource="http://www.w3.org/2001/XMLSchema#string"/>
  </owl:DatatypeProperty>
  <owl:DatatypeProperty rdf:about="http://example.org/onto/prop/google_os_config_v2_policy_orchestrator_for_organization_deleted">
    <rdfs:label>deleted</rdfs:label>
    <rdfs:comment>Output only. Indicates that this revision deletes the OS policy assignment.</rdfs:comment>
    <rdfs:domain rdf:resource="http://example.org/onto/class/google_os_config_v2_policy_orchestrator_for_organization"/>
    <rdfs:range rdf:resource="http://www.w3.org/2001/XMLSchema#string"/>
  </owl:DatatypeProperty>
  <owl:DatatypeProperty rdf:about="http://example.org/onto/prop/google_os_config_v2_policy_orchestrator_for_organization_description">
    <rdfs:label>description</rdfs:label>
    <rdfs:comment>OS policy assignment description.
Length of the description is limited to 1024 characters.</rdfs:comment>
    <rdfs:domain rdf:resource="http://example.org/onto/class/google_os_config_v2_policy_orchestrator_for_organization"/>
    <rdfs:range rdf:resource="http://www.w3.org/2001/XMLSchema#string"/>
  </owl:DatatypeProperty>
  <owl:DatatypeProperty rdf:about="http://example.org/onto/prop/google_os_config_v2_policy_orchestrator_for_organization_etag">
    <rdfs:label>etag</rdfs:label>
    <rdfs:comment>The etag for this OS policy assignment.
If this is provided on update, it must match the server's etag.</rdfs:comment>
    <rdfs:domain rdf:resource="http://example.org/onto/class/google_os_config_v2_policy_orchestrator_for_organization"/>
    <rdfs:range rdf:resource="http://www.w3.org/2001/XMLSchema#string"/>
  </owl:DatatypeProperty>
  <owl:DatatypeProperty rdf:about="http://example.org/onto/prop/google_os_config_v2_policy_orchestrator_for_organization_name">
    <rdfs:label>name</rdfs:label>
    <rdfs:comment>Resource name.

Format:
'projects/{project_number}/locations/{location}/osPolicyAssignments/{os_policy_assignment_id}'

This field is ignored when you create an OS policy assignment.</rdfs:comment>
    <rdfs:domain rdf:resource="http://example.org/onto/class/google_os_config_v2_policy_orchestrator_for_organization"/>
    <rdfs:range rdf:resource="http://www.w3.org/2001/XMLSchema#string"/>
  </owl:DatatypeProperty>
  <owl:DatatypeProperty rdf:about="http://example.org/onto/prop/google_os_config_v2_policy_orchestrator_for_organization_reconciling">
    <rdfs:label>reconciling</rdfs:label>
    <rdfs:comment>Output only. Indicates that reconciliation is in progress for the revision.
This value is 'true' when the 'rollout_state' is one of:
* IN_PROGRESS
* CANCELLING</rdfs:comment>
    <rdfs:domain rdf:resource="http://example.org/onto/class/google_os_config_v2_policy_orchestrator_for_organization"/>
    <rdfs:range rdf:resource="http://www.w3.org/2001/XMLSchema#string"/>
  </owl:DatatypeProperty>
  <owl:DatatypeProperty rdf:about="http://example.org/onto/prop/google_os_config_v2_policy_orchestrator_for_organization_revision_create_time">
    <rdfs:label>revision_create_time</rdfs:label>
    <rdfs:comment>Output only. The timestamp that the revision was created.</rdfs:comment>
    <rdfs:domain rdf:resource="http://example.org/onto/class/google_os_config_v2_policy_orchestrator_for_organization"/>
    <rdfs:range rdf:resource="http://www.w3.org/2001/XMLSchema#string"/>
  </owl:DatatypeProperty>
  <owl:DatatypeProperty rdf:about="http://example.org/onto/prop/google_os_config_v2_policy_orchestrator_for_organization_revision_id">
    <rdfs:label>revision_id</rdfs:label>
    <rdfs:comment>Output only. The assignment revision ID
A new revision is committed whenever a rollout is triggered for a OS policy
assignment</rdfs:comment>
    <rdfs:domain rdf:resource="http://example.org/onto/class/google_os_config_v2_policy_orchestrator_for_organization"/>
    <rdfs:range rdf:resource="http://www.w3.org/2001/XMLSchema#string"/>
  </owl:DatatypeProperty>
  <owl:DatatypeProperty rdf:about="http://example.org/onto/prop/google_os_config_v2_policy_orchestrator_for_organization_rollout_state">
    <rdfs:label>rollout_state</rdfs:label>
    <rdfs:comment>Output only. OS policy assignment rollout state
Possible values:
ROLLOUT_STATE_UNSPECIFIED
IN_PROGRESS
CANCELLING
CANCELLED
SUCCEEDED</rdfs:comment>
    <rdfs:domain rdf:resource="http://example.org/onto/class/google_os_config_v2_policy_orchestrator_for_organization"/>
    <rdfs:range rdf:resource="http://www.w3.org/2001/XMLSchema#string"/>
  </owl:DatatypeProperty>
  <owl:DatatypeProperty rdf:about="http://example.org/onto/prop/google_os_config_v2_policy_orchestrator_for_organization_uid">
    <rdfs:label>uid</rdfs:label>
    <rdfs:comment>Output only. Server generated unique id for the OS policy assignment resource.</rdfs:comment>
    <rdfs:domain rdf:resource="http://example.org/onto/class/google_os_config_v2_policy_orchestrator_for_organization"/>
    <rdfs:range rdf:resource="http://www.w3.org/2001/XMLSchema#string"/>
  </owl:DatatypeProperty>
  <owl:DatatypeProperty rdf:about="http://example.org/onto/prop/google_os_config_v2_policy_orchestrator_for_organization_all">
    <rdfs:label>all</rdfs:label>
    <rdfs:comment>Target all VMs in the project. If true, no other criteria is
permitted.</rdfs:comment>
    <rdfs:domain rdf:resource="http://example.org/onto/class/google_os_config_v2_policy_orchestrator_for_organization"/>
    <rdfs:range rdf:resource="http://www.w3.org/2001/XMLSchema#string"/>
  </owl:DatatypeProperty>
  <owl:DatatypeProperty rdf:about="http://example.org/onto/prop/google_os_config_v2_policy_orchestrator_for_organization_labels">
    <rdfs:label>labels</rdfs:label>
    <rdfs:comment>Labels are identified by key/value pairs in this map.
A VM should contain all the key/value pairs specified in this
map to be selected.</rdfs:comment>
    <rdfs:domain rdf:resource="http://example.org/onto/class/google_os_config_v2_policy_orchestrator_for_organization"/>
    <rdfs:range rdf:resource="http://www.w3.org/2001/XMLSchema#string"/>
  </owl:DatatypeProperty>
  <owl:DatatypeProperty rdf:about="http://example.org/onto/prop/google_os_config_v2_policy_orchestrator_for_organization_labels">
    <rdfs:label>labels</rdfs:label>
    <rdfs:comment>Labels are identified by key/value pairs in this map.
A VM should contain all the key/value pairs specified in this
map to be selected.</rdfs:comment>
    <rdfs:domain rdf:resource="http://example.org/onto/class/google_os_config_v2_policy_orchestrator_for_organization"/>
    <rdfs:range rdf:resource="http://www.w3.org/2001/XMLSchema#string"/>
  </owl:DatatypeProperty>
  <owl:DatatypeProperty rdf:about="http://example.org/onto/prop/google_os_config_v2_policy_orchestrator_for_organization_os_short_name">
    <rdfs:label>os_short_name</rdfs:label>
    <rdfs:comment>Required. The OS short name</rdfs:comment>
    <rdfs:domain rdf:resource="http://example.org/onto/class/google_os_config_v2_policy_orchestrator_for_organization"/>
    <rdfs:range rdf:resource="http://www.w3.org/2001/XMLSchema#string"/>
  </owl:DatatypeProperty>
  <owl:DatatypeProperty rdf:about="http://example.org/onto/prop/google_os_config_v2_policy_orchestrator_for_organization_os_version">
    <rdfs:label>os_version</rdfs:label>
    <rdfs:comment>The OS version

Prefix matches are supported if asterisk(*) is provided as the
last character. For example, to match all versions with a major
version of '7', specify the following value for this field '7.*'

An empty string matches all OS versions.</rdfs:comment>
    <rdfs:domain rdf:resource="http://example.org/onto/class/google_os_config_v2_policy_orchestrator_for_organization"/>
    <rdfs:range rdf:resource="http://www.w3.org/2001/XMLSchema#string"/>
  </owl:DatatypeProperty>
  <owl:DatatypeProperty rdf:about="http://example.org/onto/prop/google_os_config_v2_policy_orchestrator_for_organization_allow_no_resource_group_match">
    <rdfs:label>allow_no_resource_group_match</rdfs:label>
    <rdfs:comment>This flag determines the OS policy compliance status when none of the
resource groups within the policy are applicable for a VM. Set this value
to 'true' if the policy needs to be reported as compliant even if the
policy has nothing to validate or enforce.</rdfs:comment>
    <rdfs:domain rdf:resource="http://example.org/onto/class/google_os_config_v2_policy_orchestrator_for_organization"/>
    <rdfs:range rdf:resource="http://www.w3.org/2001/XMLSchema#string"/>
  </owl:DatatypeProperty>
  <owl:DatatypeProperty rdf:about="http://example.org/onto/prop/google_os_config_v2_policy_orchestrator_for_organization_description">
    <rdfs:label>description</rdfs:label>
    <rdfs:comment>Policy description.
Length of the description is limited to 1024 characters.</rdfs:comment>
    <rdfs:domain rdf:resource="http://example.org/onto/class/google_os_config_v2_policy_orchestrator_for_organization"/>
    <rdfs:range rdf:resource="http://www.w3.org/2001/XMLSchema#string"/>
  </owl:DatatypeProperty>
  <owl:DatatypeProperty rdf:about="http://example.org/onto/prop/google_os_config_v2_policy_orchestrator_for_organization_id">
    <rdfs:label>id</rdfs:label>
    <rdfs:comment>Required. The id of the OS policy with the following restrictions:

* Must contain only lowercase letters, numbers, and hyphens.
* Must start with a letter.
* Must be between 1-63 characters.
* Must end with a number or a letter.
* Must be unique within the assignment.</rdfs:comment>
    <rdfs:domain rdf:resource="http://example.org/onto/class/google_os_config_v2_policy_orchestrator_for_organization"/>
    <rdfs:range rdf:resource="http://www.w3.org/2001/XMLSchema#string"/>
  </owl:DatatypeProperty>
  <owl:DatatypeProperty rdf:about="http://example.org/onto/prop/google_os_config_v2_policy_orchestrator_for_organization_mode">
    <rdfs:label>mode</rdfs:label>
    <rdfs:comment>Required. Policy mode
Possible values:
MODE_UNSPECIFIED
VALIDATION
ENFORCEMENT</rdfs:comment>
    <rdfs:domain rdf:resource="http://example.org/onto/class/google_os_config_v2_policy_orchestrator_for_organization"/>
    <rdfs:range rdf:resource="http://www.w3.org/2001/XMLSchema#string"/>
  </owl:DatatypeProperty>
  <owl:DatatypeProperty rdf:about="http://example.org/onto/prop/google_os_config_v2_policy_orchestrator_for_organization_os_short_name">
    <rdfs:label>os_short_name</rdfs:label>
    <rdfs:comment>Required. The OS short name</rdfs:comment>
    <rdfs:domain rdf:resource="http://example.org/onto/class/google_os_config_v2_policy_orchestrator_for_organization"/>
    <rdfs:range rdf:resource="http://www.w3.org/2001/XMLSchema#string"/>
  </owl:DatatypeProperty>
  <owl:DatatypeProperty rdf:about="http://example.org/onto/prop/google_os_config_v2_policy_orchestrator_for_organization_os_version">
    <rdfs:label>os_version</rdfs:label>
    <rdfs:comment>The OS version

Prefix matches are supported if asterisk(*) is provided as the
last character. For example, to match all versions with a major
version of '7', specify the following value for this field '7.*'

An empty string matches all OS versions.</rdfs:comment>
    <rdfs:domain rdf:resource="http://example.org/onto/class/google_os_config_v2_policy_orchestrator_for_organization"/>
    <rdfs:range rdf:resource="http://www.w3.org/2001/XMLSchema#string"/>
  </owl:DatatypeProperty>
  <owl:DatatypeProperty rdf:about="http://example.org/onto/prop/google_os_config_v2_policy_orchestrator_for_organization_id">
    <rdfs:label>id</rdfs:label>
    <rdfs:comment>Required. The id of the resource with the following restrictions:

* Must contain only lowercase letters, numbers, and hyphens.
* Must start with a letter.
* Must be between 1-63 characters.
* Must end with a number or a letter.
* Must be unique within the OS policy.</rdfs:comment>
    <rdfs:domain rdf:resource="http://example.org/onto/class/google_os_config_v2_policy_orchestrator_for_organization"/>
    <rdfs:range rdf:resource="http://www.w3.org/2001/XMLSchema#string"/>
  </owl:DatatypeProperty>
  <owl:DatatypeProperty rdf:about="http://example.org/onto/prop/google_os_config_v2_policy_orchestrator_for_organization_args">
    <rdfs:label>args</rdfs:label>
    <rdfs:comment>Optional arguments to pass to the source during execution.</rdfs:comment>
    <rdfs:domain rdf:resource="http://example.org/onto/class/google_os_config_v2_policy_orchestrator_for_organization"/>
    <rdfs:range rdf:resource="http://www.w3.org/2001/XMLSchema#string"/>
  </owl:DatatypeProperty>
  <owl:DatatypeProperty rdf:about="http://example.org/onto/prop/google_os_config_v2_policy_orchestrator_for_organization_interpreter">
    <rdfs:label>interpreter</rdfs:label>
    <rdfs:comment>Required. The script interpreter to use.
Possible values:
INTERPRETER_UNSPECIFIED
NONE
SHELL
POWERSHELL</rdfs:comment>
    <rdfs:domain rdf:resource="http://example.org/onto/class/google_os_config_v2_policy_orchestrator_for_organization"/>
    <rdfs:range rdf:resource="http://www.w3.org/2001/XMLSchema#string"/>
  </owl:DatatypeProperty>
  <owl:DatatypeProperty rdf:about="http://example.org/onto/prop/google_os_config_v2_policy_orchestrator_for_organization_output_file_path">
    <rdfs:label>output_file_path</rdfs:label>
    <rdfs:comment>Only recorded for enforce Exec.
Path to an output file (that is created by this Exec) whose
content will be recorded in OSPolicyResourceCompliance after a
successful run. Absence or failure to read this file will result in
this ExecResource being non-compliant. Output file size is limited to
500K bytes.</rdfs:comment>
    <rdfs:domain rdf:resource="http://example.org/onto/class/google_os_config_v2_policy_orchestrator_for_organization"/>
    <rdfs:range rdf:resource="http://www.w3.org/2001/XMLSchema#string"/>
  </owl:DatatypeProperty>
  <owl:DatatypeProperty rdf:about="http://example.org/onto/prop/google_os_config_v2_policy_orchestrator_for_organization_script">
    <rdfs:label>script</rdfs:label>
    <rdfs:comment>An inline script.
The size of the script is limited to 32KiB.</rdfs:comment>
    <rdfs:domain rdf:resource="http://example.org/onto/class/google_os_config_v2_policy_orchestrator_for_organization"/>
    <rdfs:range rdf:resource="http://www.w3.org/2001/XMLSchema#string"/>
  </owl:DatatypeProperty>
  <owl:DatatypeProperty rdf:about="http://example.org/onto/prop/google_os_config_v2_policy_orchestrator_for_organization_allow_insecure">
    <rdfs:label>allow_insecure</rdfs:label>
    <rdfs:comment>Defaults to false. When false, files are subject to validations
based on the file type:

Remote: A checksum must be specified.
Cloud Storage: An object generation number must be specified.</rdfs:comment>
    <rdfs:domain rdf:resource="http://example.org/onto/class/google_os_config_v2_policy_orchestrator_for_organization"/>
    <rdfs:range rdf:resource="http://www.w3.org/2001/XMLSchema#string"/>
  </owl:DatatypeProperty>
  <owl:DatatypeProperty rdf:about="http://example.org/onto/prop/google_os_config_v2_policy_orchestrator_for_organization_local_path">
    <rdfs:label>local_path</rdfs:label>
    <rdfs:comment>A local path within the VM to use.</rdfs:comment>
    <rdfs:domain rdf:resource="http://example.org/onto/class/google_os_config_v2_policy_orchestrator_for_organization"/>
    <rdfs:range rdf:resource="http://www.w3.org/2001/XMLSchema#string"/>
  </owl:DatatypeProperty>
  <owl:DatatypeProperty rdf:about="http://example.org/onto/prop/google_os_config_v2_policy_orchestrator_for_organization_bucket">
    <rdfs:label>bucket</rdfs:label>
    <rdfs:comment>Required. Bucket of the Cloud Storage object.</rdfs:comment>
    <rdfs:domain rdf:resource="http://example.org/onto/class/google_os_config_v2_policy_orchestrator_for_organization"/>
    <rdfs:range rdf:resource="http://www.w3.org/2001/XMLSchema#string"/>
  </owl:DatatypeProperty>
  <owl:DatatypeProperty rdf:about="http://example.org/onto/prop/google_os_config_v2_policy_orchestrator_for_organization_generation">
    <rdfs:label>generation</rdfs:label>
    <rdfs:comment>Generation number of the Cloud Storage object.</rdfs:comment>
    <rdfs:domain rdf:resource="http://example.org/onto/class/google_os_config_v2_policy_orchestrator_for_organization"/>
    <rdfs:range rdf:resource="http://www.w3.org/2001/XMLSchema#string"/>
  </owl:DatatypeProperty>
  <owl:DatatypeProperty rdf:about="http://example.org/onto/prop/google_os_config_v2_policy_orchestrator_for_organization_object">
    <rdfs:label>object</rdfs:label>
    <rdfs:comment>Required. Name of the Cloud Storage object.</rdfs:comment>
    <rdfs:domain rdf:resource="http://example.org/onto/class/google_os_config_v2_policy_orchestrator_for_organization"/>
    <rdfs:range rdf:resource="http://www.w3.org/2001/XMLSchema#string"/>
  </owl:DatatypeProperty>
  <owl:DatatypeProperty rdf:about="http://example.org/onto/prop/google_os_config_v2_policy_orchestrator_for_organization_sha256_checksum">
    <rdfs:label>sha256_checksum</rdfs:label>
    <rdfs:comment>SHA256 checksum of the remote file.</rdfs:comment>
    <rdfs:domain rdf:resource="http://example.org/onto/class/google_os_config_v2_policy_orchestrator_for_organization"/>
    <rdfs:range rdf:resource="http://www.w3.org/2001/XMLSchema#string"/>
  </owl:DatatypeProperty>
  <owl:DatatypeProperty rdf:about="http://example.org/onto/prop/google_os_config_v2_policy_orchestrator_for_organization_uri">
    <rdfs:label>uri</rdfs:label>
    <rdfs:comment>Required. URI from which to fetch the object. It should contain both the
protocol and path following the format '{protocol}://{location}'.</rdfs:comment>
    <rdfs:domain rdf:resource="http://example.org/onto/class/google_os_config_v2_policy_orchestrator_for_organization"/>
    <rdfs:range rdf:resource="http://www.w3.org/2001/XMLSchema#string"/>
  </owl:DatatypeProperty>
  <owl:DatatypeProperty rdf:about="http://example.org/onto/prop/google_os_config_v2_policy_orchestrator_for_organization_args">
    <rdfs:label>args</rdfs:label>
    <rdfs:comment>Optional arguments to pass to the source during execution.</rdfs:comment>
    <rdfs:domain rdf:resource="http://example.org/onto/class/google_os_config_v2_policy_orchestrator_for_organization"/>
    <rdfs:range rdf:resource="http://www.w3.org/2001/XMLSchema#string"/>
  </owl:DatatypeProperty>
  <owl:DatatypeProperty rdf:about="http://example.org/onto/prop/google_os_config_v2_policy_orchestrator_for_organization_interpreter">
    <rdfs:label>interpreter</rdfs:label>
    <rdfs:comment>Required. The script interpreter to use.
Possible values:
INTERPRETER_UNSPECIFIED
NONE
SHELL
POWERSHELL</rdfs:comment>
    <rdfs:domain rdf:resource="http://example.org/onto/class/google_os_config_v2_policy_orchestrator_for_organization"/>
    <rdfs:range rdf:resource="http://www.w3.org/2001/XMLSchema#string"/>
  </owl:DatatypeProperty>
  <owl:DatatypeProperty rdf:about="http://example.org/onto/prop/google_os_config_v2_policy_orchestrator_for_organization_output_file_path">
    <rdfs:label>output_file_path</rdfs:label>
    <rdfs:comment>Only recorded for enforce Exec.
Path to an output file (that is created by this Exec) whose
content will be recorded in OSPolicyResourceCompliance after a
successful run. Absence or failure to read this file will result in
this ExecResource being non-compliant. Output file size is limited to
500K bytes.</rdfs:comment>
    <rdfs:domain rdf:resource="http://example.org/onto/class/google_os_config_v2_policy_orchestrator_for_organization"/>
    <rdfs:range rdf:resource="http://www.w3.org/2001/XMLSchema#string"/>
  </owl:DatatypeProperty>
  <owl:DatatypeProperty rdf:about="http://example.org/onto/prop/google_os_config_v2_policy_orchestrator_for_organization_script">
    <rdfs:label>script</rdfs:label>
    <rdfs:comment>An inline script.
The size of the script is limited to 32KiB.</rdfs:comment>
    <rdfs:domain rdf:resource="http://example.org/onto/class/google_os_config_v2_policy_orchestrator_for_organization"/>
    <rdfs:range rdf:resource="http://www.w3.org/2001/XMLSchema#string"/>
  </owl:DatatypeProperty>
  <owl:DatatypeProperty rdf:about="http://example.org/onto/prop/google_os_config_v2_policy_orchestrator_for_organization_allow_insecure">
    <rdfs:label>allow_insecure</rdfs:label>
    <rdfs:comment>Defaults to false. When false, files are subject to validations
based on the file type:

Remote: A checksum must be specified.
Cloud Storage: An object generation number must be specified.</rdfs:comment>
    <rdfs:domain rdf:resource="http://example.org/onto/class/google_os_config_v2_policy_orchestrator_for_organization"/>
    <rdfs:range rdf:resource="http://www.w3.org/2001/XMLSchema#string"/>
  </owl:DatatypeProperty>
  <owl:DatatypeProperty rdf:about="http://example.org/onto/prop/google_os_config_v2_policy_orchestrator_for_organization_local_path">
    <rdfs:label>local_path</rdfs:label>
    <rdfs:comment>A local path within the VM to use.</rdfs:comment>
    <rdfs:domain rdf:resource="http://example.org/onto/class/google_os_config_v2_policy_orchestrator_for_organization"/>
    <rdfs:range rdf:resource="http://www.w3.org/2001/XMLSchema#string"/>
  </owl:DatatypeProperty>
  <owl:DatatypeProperty rdf:about="http://example.org/onto/prop/google_os_config_v2_policy_orchestrator_for_organization_bucket">
    <rdfs:label>bucket</rdfs:label>
    <rdfs:comment>Required. Bucket of the Cloud Storage object.</rdfs:comment>
    <rdfs:domain rdf:resource="http://example.org/onto/class/google_os_config_v2_policy_orchestrator_for_organization"/>
    <rdfs:range rdf:resource="http://www.w3.org/2001/XMLSchema#string"/>
  </owl:DatatypeProperty>
  <owl:DatatypeProperty rdf:about="http://example.org/onto/prop/google_os_config_v2_policy_orchestrator_for_organization_generation">
    <rdfs:label>generation</rdfs:label>
    <rdfs:comment>Generation number of the Cloud Storage object.</rdfs:comment>
    <rdfs:domain rdf:resource="http://example.org/onto/class/google_os_config_v2_policy_orchestrator_for_organization"/>
    <rdfs:range rdf:resource="http://www.w3.org/2001/XMLSchema#string"/>
  </owl:DatatypeProperty>
  <owl:DatatypeProperty rdf:about="http://example.org/onto/prop/google_os_config_v2_policy_orchestrator_for_organization_object">
    <rdfs:label>object</rdfs:label>
    <rdfs:comment>Required. Name of the Cloud Storage object.</rdfs:comment>
    <rdfs:domain rdf:resource="http://example.org/onto/class/google_os_config_v2_policy_orchestrator_for_organization"/>
    <rdfs:range rdf:resource="http://www.w3.org/2001/XMLSchema#string"/>
  </owl:DatatypeProperty>
  <owl:DatatypeProperty rdf:about="http://example.org/onto/prop/google_os_config_v2_policy_orchestrator_for_organization_sha256_checksum">
    <rdfs:label>sha256_checksum</rdfs:label>
    <rdfs:comment>SHA256 checksum of the remote file.</rdfs:comment>
    <rdfs:domain rdf:resource="http://example.org/onto/class/google_os_config_v2_policy_orchestrator_for_organization"/>
    <rdfs:range rdf:resource="http://www.w3.org/2001/XMLSchema#string"/>
  </owl:DatatypeProperty>
  <owl:DatatypeProperty rdf:about="http://example.org/onto/prop/google_os_config_v2_policy_orchestrator_for_organization_uri">
    <rdfs:label>uri</rdfs:label>
    <rdfs:comment>Required. URI from which to fetch the object. It should contain both the
protocol and path following the format '{protocol}://{location}'.</rdfs:comment>
    <rdfs:domain rdf:resource="http://example.org/onto/class/google_os_config_v2_policy_orchestrator_for_organization"/>
    <rdfs:range rdf:resource="http://www.w3.org/2001/XMLSchema#string"/>
  </owl:DatatypeProperty>
  <owl:DatatypeProperty rdf:about="http://example.org/onto/prop/google_os_config_v2_policy_orchestrator_for_organization_content">
    <rdfs:label>content</rdfs:label>
    <rdfs:comment>A a file with this content.
The size of the content is limited to 32KiB.</rdfs:comment>
    <rdfs:domain rdf:resource="http://example.org/onto/class/google_os_config_v2_policy_orchestrator_for_organization"/>
    <rdfs:range rdf:resource="http://www.w3.org/2001/XMLSchema#string"/>
  </owl:DatatypeProperty>
  <owl:DatatypeProperty rdf:about="http://example.org/onto/prop/google_os_config_v2_policy_orchestrator_for_organization_path">
    <rdfs:label>path</rdfs:label>
    <rdfs:comment>Required. The absolute path of the file within the VM.</rdfs:comment>
    <rdfs:domain rdf:resource="http://example.org/onto/class/google_os_config_v2_policy_orchestrator_for_organization"/>
    <rdfs:range rdf:resource="http://www.w3.org/2001/XMLSchema#string"/>
  </owl:DatatypeProperty>
  <owl:DatatypeProperty rdf:about="http://example.org/onto/prop/google_os_config_v2_policy_orchestrator_for_organization_permissions">
    <rdfs:label>permissions</rdfs:label>
    <rdfs:comment>Consists of three octal digits which represent, in
order, the permissions of the owner, group, and other users for the
file (similarly to the numeric mode used in the linux chmod
utility). Each digit represents a three bit number with the 4 bit
corresponding to the read permissions, the 2 bit corresponds to the
write bit, and the one bit corresponds to the execute permission.
Default behavior is 755.

Below are some examples of permissions and their associated values:
read, write, and execute: 7
read and execute: 5
read and write: 6
read only: 4</rdfs:comment>
    <rdfs:domain rdf:resource="http://example.org/onto/class/google_os_config_v2_policy_orchestrator_for_organization"/>
    <rdfs:range rdf:resource="http://www.w3.org/2001/XMLSchema#string"/>
  </owl:DatatypeProperty>
  <owl:DatatypeProperty rdf:about="http://example.org/onto/prop/google_os_config_v2_policy_orchestrator_for_organization_state">
    <rdfs:label>state</rdfs:label>
    <rdfs:comment>Required. Desired state of the file.
Possible values:
DESIRED_STATE_UNSPECIFIED
PRESENT
ABSENT
CONTENTS_MATCH</rdfs:comment>
    <rdfs:domain rdf:resource="http://example.org/onto/class/google_os_config_v2_policy_orchestrator_for_organization"/>
    <rdfs:range rdf:resource="http://www.w3.org/2001/XMLSchema#string"/>
  </owl:DatatypeProperty>
  <owl:DatatypeProperty rdf:about="http://example.org/onto/prop/google_os_config_v2_policy_orchestrator_for_organization_allow_insecure">
    <rdfs:label>allow_insecure</rdfs:label>
    <rdfs:comment>Defaults to false. When false, files are subject to validations
based on the file type:

Remote: A checksum must be specified.
Cloud Storage: An object generation number must be specified.</rdfs:comment>
    <rdfs:domain rdf:resource="http://example.org/onto/class/google_os_config_v2_policy_orchestrator_for_organization"/>
    <rdfs:range rdf:resource="http://www.w3.org/2001/XMLSchema#string"/>
  </owl:DatatypeProperty>
  <owl:DatatypeProperty rdf:about="http://example.org/onto/prop/google_os_config_v2_policy_orchestrator_for_organization_local_path">
    <rdfs:label>local_path</rdfs:label>
    <rdfs:comment>A local path within the VM to use.</rdfs:comment>
    <rdfs:domain rdf:resource="http://example.org/onto/class/google_os_config_v2_policy_orchestrator_for_organization"/>
    <rdfs:range rdf:resource="http://www.w3.org/2001/XMLSchema#string"/>
  </owl:DatatypeProperty>
  <owl:DatatypeProperty rdf:about="http://example.org/onto/prop/google_os_config_v2_policy_orchestrator_for_organization_bucket">
    <rdfs:label>bucket</rdfs:label>
    <rdfs:comment>Required. Bucket of the Cloud Storage object.</rdfs:comment>
    <rdfs:domain rdf:resource="http://example.org/onto/class/google_os_config_v2_policy_orchestrator_for_organization"/>
    <rdfs:range rdf:resource="http://www.w3.org/2001/XMLSchema#string"/>
  </owl:DatatypeProperty>
  <owl:DatatypeProperty rdf:about="http://example.org/onto/prop/google_os_config_v2_policy_orchestrator_for_organization_generation">
    <rdfs:label>generation</rdfs:label>
    <rdfs:comment>Generation number of the Cloud Storage object.</rdfs:comment>
    <rdfs:domain rdf:resource="http://example.org/onto/class/google_os_config_v2_policy_orchestrator_for_organization"/>
    <rdfs:range rdf:resource="http://www.w3.org/2001/XMLSchema#string"/>
  </owl:DatatypeProperty>
  <owl:DatatypeProperty rdf:about="http://example.org/onto/prop/google_os_config_v2_policy_orchestrator_for_organization_object">
    <rdfs:label>object</rdfs:label>
    <rdfs:comment>Required. Name of the Cloud Storage object.</rdfs:comment>
    <rdfs:domain rdf:resource="http://example.org/onto/class/google_os_config_v2_policy_orchestrator_for_organization"/>
    <rdfs:range rdf:resource="http://www.w3.org/2001/XMLSchema#string"/>
  </owl:DatatypeProperty>
  <owl:DatatypeProperty rdf:about="http://example.org/onto/prop/google_os_config_v2_policy_orchestrator_for_organization_sha256_checksum">
    <rdfs:label>sha256_checksum</rdfs:label>
    <rdfs:comment>SHA256 checksum of the remote file.</rdfs:comment>
    <rdfs:domain rdf:resource="http://example.org/onto/class/google_os_config_v2_policy_orchestrator_for_organization"/>
    <rdfs:range rdf:resource="http://www.w3.org/2001/XMLSchema#string"/>
  </owl:DatatypeProperty>
  <owl:DatatypeProperty rdf:about="http://example.org/onto/prop/google_os_config_v2_policy_orchestrator_for_organization_uri">
    <rdfs:label>uri</rdfs:label>
    <rdfs:comment>Required. URI from which to fetch the object. It should contain both the
protocol and path following the format '{protocol}://{location}'.</rdfs:comment>
    <rdfs:domain rdf:resource="http://example.org/onto/class/google_os_config_v2_policy_orchestrator_for_organization"/>
    <rdfs:range rdf:resource="http://www.w3.org/2001/XMLSchema#string"/>
  </owl:DatatypeProperty>
  <owl:DatatypeProperty rdf:about="http://example.org/onto/prop/google_os_config_v2_policy_orchestrator_for_organization_desired_state">
    <rdfs:label>desired_state</rdfs:label>
    <rdfs:comment>Required. The desired state the agent should maintain for this package.
Possible values:
DESIRED_STATE_UNSPECIFIED
INSTALLED
REMOVED</rdfs:comment>
    <rdfs:domain rdf:resource="http://example.org/onto/class/google_os_config_v2_policy_orchestrator_for_organization"/>
    <rdfs:range rdf:resource="http://www.w3.org/2001/XMLSchema#string"/>
  </owl:DatatypeProperty>
  <owl:DatatypeProperty rdf:about="http://example.org/onto/prop/google_os_config_v2_policy_orchestrator_for_organization_name">
    <rdfs:label>name</rdfs:label>
    <rdfs:comment>Required. Package name.</rdfs:comment>
    <rdfs:domain rdf:resource="http://example.org/onto/class/google_os_config_v2_policy_orchestrator_for_organization"/>
    <rdfs:range rdf:resource="http://www.w3.org/2001/XMLSchema#string"/>
  </owl:DatatypeProperty>
  <owl:DatatypeProperty rdf:about="http://example.org/onto/prop/google_os_config_v2_policy_orchestrator_for_organization_pull_deps">
    <rdfs:label>pull_deps</rdfs:label>
    <rdfs:comment>Whether dependencies should also be installed.
- install when false: 'dpkg -i package'
- install when true: 'apt-get update && apt-get -y install
package.deb'</rdfs:comment>
    <rdfs:domain rdf:resource="http://example.org/onto/class/google_os_config_v2_policy_orchestrator_for_organization"/>
    <rdfs:range rdf:resource="http://www.w3.org/2001/XMLSchema#string"/>
  </owl:DatatypeProperty>
  <owl:DatatypeProperty rdf:about="http://example.org/onto/prop/google_os_config_v2_policy_orchestrator_for_organization_allow_insecure">
    <rdfs:label>allow_insecure</rdfs:label>
    <rdfs:comment>Defaults to false. When false, files are subject to validations
based on the file type:

Remote: A checksum must be specified.
Cloud Storage: An object generation number must be specified.</rdfs:comment>
    <rdfs:domain rdf:resource="http://example.org/onto/class/google_os_config_v2_policy_orchestrator_for_organization"/>
    <rdfs:range rdf:resource="http://www.w3.org/2001/XMLSchema#string"/>
  </owl:DatatypeProperty>
  <owl:DatatypeProperty rdf:about="http://example.org/onto/prop/google_os_config_v2_policy_orchestrator_for_organization_local_path">
    <rdfs:label>local_path</rdfs:label>
    <rdfs:comment>A local path within the VM to use.</rdfs:comment>
    <rdfs:domain rdf:resource="http://example.org/onto/class/google_os_config_v2_policy_orchestrator_for_organization"/>
    <rdfs:range rdf:resource="http://www.w3.org/2001/XMLSchema#string"/>
  </owl:DatatypeProperty>
  <owl:DatatypeProperty rdf:about="http://example.org/onto/prop/google_os_config_v2_policy_orchestrator_for_organization_bucket">
    <rdfs:label>bucket</rdfs:label>
    <rdfs:comment>Required. Bucket of the Cloud Storage object.</rdfs:comment>
    <rdfs:domain rdf:resource="http://example.org/onto/class/google_os_config_v2_policy_orchestrator_for_organization"/>
    <rdfs:range rdf:resource="http://www.w3.org/2001/XMLSchema#string"/>
  </owl:DatatypeProperty>
  <owl:DatatypeProperty rdf:about="http://example.org/onto/prop/google_os_config_v2_policy_orchestrator_for_organization_generation">
    <rdfs:label>generation</rdfs:label>
    <rdfs:comment>Generation number of the Cloud Storage object.</rdfs:comment>
    <rdfs:domain rdf:resource="http://example.org/onto/class/google_os_config_v2_policy_orchestrator_for_organization"/>
    <rdfs:range rdf:resource="http://www.w3.org/2001/XMLSchema#string"/>
  </owl:DatatypeProperty>
  <owl:DatatypeProperty rdf:about="http://example.org/onto/prop/google_os_config_v2_policy_orchestrator_for_organization_object">
    <rdfs:label>object</rdfs:label>
    <rdfs:comment>Required. Name of the Cloud Storage object.</rdfs:comment>
    <rdfs:domain rdf:resource="http://example.org/onto/class/google_os_config_v2_policy_orchestrator_for_organization"/>
    <rdfs:range rdf:resource="http://www.w3.org/2001/XMLSchema#string"/>
  </owl:DatatypeProperty>
  <owl:DatatypeProperty rdf:about="http://example.org/onto/prop/google_os_config_v2_policy_orchestrator_for_organization_sha256_checksum">
    <rdfs:label>sha256_checksum</rdfs:label>
    <rdfs:comment>SHA256 checksum of the remote file.</rdfs:comment>
    <rdfs:domain rdf:resource="http://example.org/onto/class/google_os_config_v2_policy_orchestrator_for_organization"/>
    <rdfs:range rdf:resource="http://www.w3.org/2001/XMLSchema#string"/>
  </owl:DatatypeProperty>
  <owl:DatatypeProperty rdf:about="http://example.org/onto/prop/google_os_config_v2_policy_orchestrator_for_organization_uri">
    <rdfs:label>uri</rdfs:label>
    <rdfs:comment>Required. URI from which to fetch the object. It should contain both the
protocol and path following the format '{protocol}://{location}'.</rdfs:comment>
    <rdfs:domain rdf:resource="http://example.org/onto/class/google_os_config_v2_policy_orchestrator_for_organization"/>
    <rdfs:range rdf:resource="http://www.w3.org/2001/XMLSchema#string"/>
  </owl:DatatypeProperty>
  <owl:DatatypeProperty rdf:about="http://example.org/onto/prop/google_os_config_v2_policy_orchestrator_for_organization_name">
    <rdfs:label>name</rdfs:label>
    <rdfs:comment>Required. Package name.</rdfs:comment>
    <rdfs:domain rdf:resource="http://example.org/onto/class/google_os_config_v2_policy_orchestrator_for_organization"/>
    <rdfs:range rdf:resource="http://www.w3.org/2001/XMLSchema#string"/>
  </owl:DatatypeProperty>
  <owl:DatatypeProperty rdf:about="http://example.org/onto/prop/google_os_config_v2_policy_orchestrator_for_organization_properties">
    <rdfs:label>properties</rdfs:label>
    <rdfs:comment>Additional properties to use during installation.
This should be in the format of Property=Setting.
Appended to the defaults of 'ACTION=INSTALL
REBOOT=ReallySuppress'.</rdfs:comment>
    <rdfs:domain rdf:resource="http://example.org/onto/class/google_os_config_v2_policy_orchestrator_for_organization"/>
    <rdfs:range rdf:resource="http://www.w3.org/2001/XMLSchema#string"/>
  </owl:DatatypeProperty>
  <owl:DatatypeProperty rdf:about="http://example.org/onto/prop/google_os_config_v2_policy_orchestrator_for_organization_allow_insecure">
    <rdfs:label>allow_insecure</rdfs:label>
    <rdfs:comment>Defaults to false. When false, files are subject to validations
based on the file type:

Remote: A checksum must be specified.
Cloud Storage: An object generation number must be specified.</rdfs:comment>
    <rdfs:domain rdf:resource="http://example.org/onto/class/google_os_config_v2_policy_orchestrator_for_organization"/>
    <rdfs:range rdf:resource="http://www.w3.org/2001/XMLSchema#string"/>
  </owl:DatatypeProperty>
  <owl:DatatypeProperty rdf:about="http://example.org/onto/prop/google_os_config_v2_policy_orchestrator_for_organization_local_path">
    <rdfs:label>local_path</rdfs:label>
    <rdfs:comment>A local path within the VM to use.</rdfs:comment>
    <rdfs:domain rdf:resource="http://example.org/onto/class/google_os_config_v2_policy_orchestrator_for_organization"/>
    <rdfs:range rdf:resource="http://www.w3.org/2001/XMLSchema#string"/>
  </owl:DatatypeProperty>
  <owl:DatatypeProperty rdf:about="http://example.org/onto/prop/google_os_config_v2_policy_orchestrator_for_organization_bucket">
    <rdfs:label>bucket</rdfs:label>
    <rdfs:comment>Required. Bucket of the Cloud Storage object.</rdfs:comment>
    <rdfs:domain rdf:resource="http://example.org/onto/class/google_os_config_v2_policy_orchestrator_for_organization"/>
    <rdfs:range rdf:resource="http://www.w3.org/2001/XMLSchema#string"/>
  </owl:DatatypeProperty>
  <owl:DatatypeProperty rdf:about="http://example.org/onto/prop/google_os_config_v2_policy_orchestrator_for_organization_generation">
    <rdfs:label>generation</rdfs:label>
    <rdfs:comment>Generation number of the Cloud Storage object.</rdfs:comment>
    <rdfs:domain rdf:resource="http://example.org/onto/class/google_os_config_v2_policy_orchestrator_for_organization"/>
    <rdfs:range rdf:resource="http://www.w3.org/2001/XMLSchema#string"/>
  </owl:DatatypeProperty>
  <owl:DatatypeProperty rdf:about="http://example.org/onto/prop/google_os_config_v2_policy_orchestrator_for_organization_object">
    <rdfs:label>object</rdfs:label>
    <rdfs:comment>Required. Name of the Cloud Storage object.</rdfs:comment>
    <rdfs:domain rdf:resource="http://example.org/onto/class/google_os_config_v2_policy_orchestrator_for_organization"/>
    <rdfs:range rdf:resource="http://www.w3.org/2001/XMLSchema#string"/>
  </owl:DatatypeProperty>
  <owl:DatatypeProperty rdf:about="http://example.org/onto/prop/google_os_config_v2_policy_orchestrator_for_organization_sha256_checksum">
    <rdfs:label>sha256_checksum</rdfs:label>
    <rdfs:comment>SHA256 checksum of the remote file.</rdfs:comment>
    <rdfs:domain rdf:resource="http://example.org/onto/class/google_os_config_v2_policy_orchestrator_for_organization"/>
    <rdfs:range rdf:resource="http://www.w3.org/2001/XMLSchema#string"/>
  </owl:DatatypeProperty>
  <owl:DatatypeProperty rdf:about="http://example.org/onto/prop/google_os_config_v2_policy_orchestrator_for_organization_uri">
    <rdfs:label>uri</rdfs:label>
    <rdfs:comment>Required. URI from which to fetch the object. It should contain both the
protocol and path following the format '{protocol}://{location}'.</rdfs:comment>
    <rdfs:domain rdf:resource="http://example.org/onto/class/google_os_config_v2_policy_orchestrator_for_organization"/>
    <rdfs:range rdf:resource="http://www.w3.org/2001/XMLSchema#string"/>
  </owl:DatatypeProperty>
  <owl:DatatypeProperty rdf:about="http://example.org/onto/prop/google_os_config_v2_policy_orchestrator_for_organization_pull_deps">
    <rdfs:label>pull_deps</rdfs:label>
    <rdfs:comment>Whether dependencies should also be installed.
- install when false: 'rpm --upgrade --replacepkgs package.rpm'
- install when true: 'yum -y install package.rpm' or
'zypper -y install package.rpm'</rdfs:comment>
    <rdfs:domain rdf:resource="http://example.org/onto/class/google_os_config_v2_policy_orchestrator_for_organization"/>
    <rdfs:range rdf:resource="http://www.w3.org/2001/XMLSchema#string"/>
  </owl:DatatypeProperty>
  <owl:DatatypeProperty rdf:about="http://example.org/onto/prop/google_os_config_v2_policy_orchestrator_for_organization_allow_insecure">
    <rdfs:label>allow_insecure</rdfs:label>
    <rdfs:comment>Defaults to false. When false, files are subject to validations
based on the file type:

Remote: A checksum must be specified.
Cloud Storage: An object generation number must be specified.</rdfs:comment>
    <rdfs:domain rdf:resource="http://example.org/onto/class/google_os_config_v2_policy_orchestrator_for_organization"/>
    <rdfs:range rdf:resource="http://www.w3.org/2001/XMLSchema#string"/>
  </owl:DatatypeProperty>
  <owl:DatatypeProperty rdf:about="http://example.org/onto/prop/google_os_config_v2_policy_orchestrator_for_organization_local_path">
    <rdfs:label>local_path</rdfs:label>
    <rdfs:comment>A local path within the VM to use.</rdfs:comment>
    <rdfs:domain rdf:resource="http://example.org/onto/class/google_os_config_v2_policy_orchestrator_for_organization"/>
    <rdfs:range rdf:resource="http://www.w3.org/2001/XMLSchema#string"/>
  </owl:DatatypeProperty>
  <owl:DatatypeProperty rdf:about="http://example.org/onto/prop/google_os_config_v2_policy_orchestrator_for_organization_bucket">
    <rdfs:label>bucket</rdfs:label>
    <rdfs:comment>Required. Bucket of the Cloud Storage object.</rdfs:comment>
    <rdfs:domain rdf:resource="http://example.org/onto/class/google_os_config_v2_policy_orchestrator_for_organization"/>
    <rdfs:range rdf:resource="http://www.w3.org/2001/XMLSchema#string"/>
  </owl:DatatypeProperty>
  <owl:DatatypeProperty rdf:about="http://example.org/onto/prop/google_os_config_v2_policy_orchestrator_for_organization_generation">
    <rdfs:label>generation</rdfs:label>
    <rdfs:comment>Generation number of the Cloud Storage object.</rdfs:comment>
    <rdfs:domain rdf:resource="http://example.org/onto/class/google_os_config_v2_policy_orchestrator_for_organization"/>
    <rdfs:range rdf:resource="http://www.w3.org/2001/XMLSchema#string"/>
  </owl:DatatypeProperty>
  <owl:DatatypeProperty rdf:about="http://example.org/onto/prop/google_os_config_v2_policy_orchestrator_for_organization_object">
    <rdfs:label>object</rdfs:label>
    <rdfs:comment>Required. Name of the Cloud Storage object.</rdfs:comment>
    <rdfs:domain rdf:resource="http://example.org/onto/class/google_os_config_v2_policy_orchestrator_for_organization"/>
    <rdfs:range rdf:resource="http://www.w3.org/2001/XMLSchema#string"/>
  </owl:DatatypeProperty>
  <owl:DatatypeProperty rdf:about="http://example.org/onto/prop/google_os_config_v2_policy_orchestrator_for_organization_sha256_checksum">
    <rdfs:label>sha256_checksum</rdfs:label>
    <rdfs:comment>SHA256 checksum of the remote file.</rdfs:comment>
    <rdfs:domain rdf:resource="http://example.org/onto/class/google_os_config_v2_policy_orchestrator_for_organization"/>
    <rdfs:range rdf:resource="http://www.w3.org/2001/XMLSchema#string"/>
  </owl:DatatypeProperty>
  <owl:DatatypeProperty rdf:about="http://example.org/onto/prop/google_os_config_v2_policy_orchestrator_for_organization_uri">
    <rdfs:label>uri</rdfs:label>
    <rdfs:comment>Required. URI from which to fetch the object. It should contain both the
protocol and path following the format '{protocol}://{location}'.</rdfs:comment>
    <rdfs:domain rdf:resource="http://example.org/onto/class/google_os_config_v2_policy_orchestrator_for_organization"/>
    <rdfs:range rdf:resource="http://www.w3.org/2001/XMLSchema#string"/>
  </owl:DatatypeProperty>
  <owl:DatatypeProperty rdf:about="http://example.org/onto/prop/google_os_config_v2_policy_orchestrator_for_organization_name">
    <rdfs:label>name</rdfs:label>
    <rdfs:comment>Required. Package name.</rdfs:comment>
    <rdfs:domain rdf:resource="http://example.org/onto/class/google_os_config_v2_policy_orchestrator_for_organization"/>
    <rdfs:range rdf:resource="http://www.w3.org/2001/XMLSchema#string"/>
  </owl:DatatypeProperty>
  <owl:DatatypeProperty rdf:about="http://example.org/onto/prop/google_os_config_v2_policy_orchestrator_for_organization_name">
    <rdfs:label>name</rdfs:label>
    <rdfs:comment>Required. Package name.</rdfs:comment>
    <rdfs:domain rdf:resource="http://example.org/onto/class/google_os_config_v2_policy_orchestrator_for_organization"/>
    <rdfs:range rdf:resource="http://www.w3.org/2001/XMLSchema#string"/>
  </owl:DatatypeProperty>
  <owl:DatatypeProperty rdf:about="http://example.org/onto/prop/google_os_config_v2_policy_orchestrator_for_organization_archive_type">
    <rdfs:label>archive_type</rdfs:label>
    <rdfs:comment>Required. Type of archive files in this repository.
Possible values:
ARCHIVE_TYPE_UNSPECIFIED
DEB
DEB_SRC</rdfs:comment>
    <rdfs:domain rdf:resource="http://example.org/onto/class/google_os_config_v2_policy_orchestrator_for_organization"/>
    <rdfs:range rdf:resource="http://www.w3.org/2001/XMLSchema#string"/>
  </owl:DatatypeProperty>
  <owl:DatatypeProperty rdf:about="http://example.org/onto/prop/google_os_config_v2_policy_orchestrator_for_organization_components">
    <rdfs:label>components</rdfs:label>
    <rdfs:comment>Required. List of components for this repository. Must contain at least one
item.</rdfs:comment>
    <rdfs:domain rdf:resource="http://example.org/onto/class/google_os_config_v2_policy_orchestrator_for_organization"/>
    <rdfs:range rdf:resource="http://www.w3.org/2001/XMLSchema#string"/>
  </owl:DatatypeProperty>
  <owl:DatatypeProperty rdf:about="http://example.org/onto/prop/google_os_config_v2_policy_orchestrator_for_organization_distribution">
    <rdfs:label>distribution</rdfs:label>
    <rdfs:comment>Required. Distribution of this repository.</rdfs:comment>
    <rdfs:domain rdf:resource="http://example.org/onto/class/google_os_config_v2_policy_orchestrator_for_organization"/>
    <rdfs:range rdf:resource="http://www.w3.org/2001/XMLSchema#string"/>
  </owl:DatatypeProperty>
  <owl:DatatypeProperty rdf:about="http://example.org/onto/prop/google_os_config_v2_policy_orchestrator_for_organization_gpg_key">
    <rdfs:label>gpg_key</rdfs:label>
    <rdfs:comment>URI of the key file for this repository. The agent maintains a
keyring at '/etc/apt/trusted.gpg.d/osconfig_agent_managed.gpg'.</rdfs:comment>
    <rdfs:domain rdf:resource="http://example.org/onto/class/google_os_config_v2_policy_orchestrator_for_organization"/>
    <rdfs:range rdf:resource="http://www.w3.org/2001/XMLSchema#string"/>
  </owl:DatatypeProperty>
  <owl:DatatypeProperty rdf:about="http://example.org/onto/prop/google_os_config_v2_policy_orchestrator_for_organization_uri">
    <rdfs:label>uri</rdfs:label>
    <rdfs:comment>Required. URI for this repository.</rdfs:comment>
    <rdfs:domain rdf:resource="http://example.org/onto/class/google_os_config_v2_policy_orchestrator_for_organization"/>
    <rdfs:range rdf:resource="http://www.w3.org/2001/XMLSchema#string"/>
  </owl:DatatypeProperty>
  <owl:DatatypeProperty rdf:about="http://example.org/onto/prop/google_os_config_v2_policy_orchestrator_for_organization_name">
    <rdfs:label>name</rdfs:label>
    <rdfs:comment>Required. The name of the repository.</rdfs:comment>
    <rdfs:domain rdf:resource="http://example.org/onto/class/google_os_config_v2_policy_orchestrator_for_organization"/>
    <rdfs:range rdf:resource="http://www.w3.org/2001/XMLSchema#string"/>
  </owl:DatatypeProperty>
  <owl:DatatypeProperty rdf:about="http://example.org/onto/prop/google_os_config_v2_policy_orchestrator_for_organization_url">
    <rdfs:label>url</rdfs:label>
    <rdfs:comment>Required. The url of the repository.</rdfs:comment>
    <rdfs:domain rdf:resource="http://example.org/onto/class/google_os_config_v2_policy_orchestrator_for_organization"/>
    <rdfs:range rdf:resource="http://www.w3.org/2001/XMLSchema#string"/>
  </owl:DatatypeProperty>
  <owl:DatatypeProperty rdf:about="http://example.org/onto/prop/google_os_config_v2_policy_orchestrator_for_organization_base_url">
    <rdfs:label>base_url</rdfs:label>
    <rdfs:comment>Required. The location of the repository directory.</rdfs:comment>
    <rdfs:domain rdf:resource="http://example.org/onto/class/google_os_config_v2_policy_orchestrator_for_organization"/>
    <rdfs:range rdf:resource="http://www.w3.org/2001/XMLSchema#string"/>
  </owl:DatatypeProperty>
  <owl:DatatypeProperty rdf:about="http://example.org/onto/prop/google_os_config_v2_policy_orchestrator_for_organization_display_name">
    <rdfs:label>display_name</rdfs:label>
    <rdfs:comment>The display name of the repository.</rdfs:comment>
    <rdfs:domain rdf:resource="http://example.org/onto/class/google_os_config_v2_policy_orchestrator_for_organization"/>
    <rdfs:range rdf:resource="http://www.w3.org/2001/XMLSchema#string"/>
  </owl:DatatypeProperty>
  <owl:DatatypeProperty rdf:about="http://example.org/onto/prop/google_os_config_v2_policy_orchestrator_for_organization_gpg_keys">
    <rdfs:label>gpg_keys</rdfs:label>
    <rdfs:comment>URIs of GPG keys.</rdfs:comment>
    <rdfs:domain rdf:resource="http://example.org/onto/class/google_os_config_v2_policy_orchestrator_for_organization"/>
    <rdfs:range rdf:resource="http://www.w3.org/2001/XMLSchema#string"/>
  </owl:DatatypeProperty>
  <owl:DatatypeProperty rdf:about="http://example.org/onto/prop/google_os_config_v2_policy_orchestrator_for_organization_id">
    <rdfs:label>id</rdfs:label>
    <rdfs:comment>Required. A one word, unique name for this repository. This is  the 'repo
id' in the yum config file and also the 'display_name' if
'display_name' is omitted. This id is also used as the unique
identifier when checking for resource conflicts.</rdfs:comment>
    <rdfs:domain rdf:resource="http://example.org/onto/class/google_os_config_v2_policy_orchestrator_for_organization"/>
    <rdfs:range rdf:resource="http://www.w3.org/2001/XMLSchema#string"/>
  </owl:DatatypeProperty>
  <owl:DatatypeProperty rdf:about="http://example.org/onto/prop/google_os_config_v2_policy_orchestrator_for_organization_base_url">
    <rdfs:label>base_url</rdfs:label>
    <rdfs:comment>Required. The location of the repository directory.</rdfs:comment>
    <rdfs:domain rdf:resource="http://example.org/onto/class/google_os_config_v2_policy_orchestrator_for_organization"/>
    <rdfs:range rdf:resource="http://www.w3.org/2001/XMLSchema#string"/>
  </owl:DatatypeProperty>
  <owl:DatatypeProperty rdf:about="http://example.org/onto/prop/google_os_config_v2_policy_orchestrator_for_organization_display_name">
    <rdfs:label>display_name</rdfs:label>
    <rdfs:comment>The display name of the repository.</rdfs:comment>
    <rdfs:domain rdf:resource="http://example.org/onto/class/google_os_config_v2_policy_orchestrator_for_organization"/>
    <rdfs:range rdf:resource="http://www.w3.org/2001/XMLSchema#string"/>
  </owl:DatatypeProperty>
  <owl:DatatypeProperty rdf:about="http://example.org/onto/prop/google_os_config_v2_policy_orchestrator_for_organization_gpg_keys">
    <rdfs:label>gpg_keys</rdfs:label>
    <rdfs:comment>URIs of GPG keys.</rdfs:comment>
    <rdfs:domain rdf:resource="http://example.org/onto/class/google_os_config_v2_policy_orchestrator_for_organization"/>
    <rdfs:range rdf:resource="http://www.w3.org/2001/XMLSchema#string"/>
  </owl:DatatypeProperty>
  <owl:DatatypeProperty rdf:about="http://example.org/onto/prop/google_os_config_v2_policy_orchestrator_for_organization_id">
    <rdfs:label>id</rdfs:label>
    <rdfs:comment>Required. A one word, unique name for this repository. This is the 'repo
id' in the zypper config file and also the 'display_name' if
'display_name' is omitted. This id is also used as the unique
identifier when checking for GuestPolicy conflicts.</rdfs:comment>
    <rdfs:domain rdf:resource="http://example.org/onto/class/google_os_config_v2_policy_orchestrator_for_organization"/>
    <rdfs:range rdf:resource="http://www.w3.org/2001/XMLSchema#string"/>
  </owl:DatatypeProperty>
  <owl:DatatypeProperty rdf:about="http://example.org/onto/prop/google_os_config_v2_policy_orchestrator_for_organization_min_wait_duration">
    <rdfs:label>min_wait_duration</rdfs:label>
    <rdfs:comment>Required. This determines the minimum duration of time to wait after the
configuration changes are applied through the current rollout. A
VM continues to count towards the 'disruption_budget' at least
until this duration of time has passed after configuration changes are
applied.</rdfs:comment>
    <rdfs:domain rdf:resource="http://example.org/onto/class/google_os_config_v2_policy_orchestrator_for_organization"/>
    <rdfs:range rdf:resource="http://www.w3.org/2001/XMLSchema#string"/>
  </owl:DatatypeProperty>
  <owl:DatatypeProperty rdf:about="http://example.org/onto/prop/google_os_config_v2_policy_orchestrator_for_organization_fixed">
    <rdfs:label>fixed</rdfs:label>
    <rdfs:comment>Specifies a fixed value.</rdfs:comment>
    <rdfs:domain rdf:resource="http://example.org/onto/class/google_os_config_v2_policy_orchestrator_for_organization"/>
    <rdfs:range rdf:resource="http://www.w3.org/2001/XMLSchema#string"/>
  </owl:DatatypeProperty>
  <owl:DatatypeProperty rdf:about="http://example.org/onto/prop/google_os_config_v2_policy_orchestrator_for_organization_percent">
    <rdfs:label>percent</rdfs:label>
    <rdfs:comment>Specifies the relative value defined as a percentage, which will be
multiplied by a reference value.</rdfs:comment>
    <rdfs:domain rdf:resource="http://example.org/onto/class/google_os_config_v2_policy_orchestrator_for_organization"/>
    <rdfs:range rdf:resource="http://www.w3.org/2001/XMLSchema#string"/>
  </owl:DatatypeProperty>
  <owl:DatatypeProperty rdf:about="http://example.org/onto/prop/google_os_config_v2_policy_orchestrator_for_organization_included_locations">
    <rdfs:label>included_locations</rdfs:label>
    <rdfs:comment>Optional. Names of the locations in scope.
Format: 'us-central1-a'</rdfs:comment>
    <rdfs:domain rdf:resource="http://example.org/onto/class/google_os_config_v2_policy_orchestrator_for_organization"/>
    <rdfs:range rdf:resource="http://www.w3.org/2001/XMLSchema#string"/>
  </owl:DatatypeProperty>
  <owl:DatatypeProperty rdf:about="http://example.org/onto/prop/google_os_config_v2_policy_orchestrator_for_organization_included_folders">
    <rdfs:label>included_folders</rdfs:label>
    <rdfs:comment>Optional. Names of the folders in scope.
Format: 'folders/{folder_id}'</rdfs:comment>
    <rdfs:domain rdf:resource="http://example.org/onto/class/google_os_config_v2_policy_orchestrator_for_organization"/>
    <rdfs:range rdf:resource="http://www.w3.org/2001/XMLSchema#string"/>
  </owl:DatatypeProperty>
  <owl:DatatypeProperty rdf:about="http://example.org/onto/prop/google_os_config_v2_policy_orchestrator_for_organization_included_projects">
    <rdfs:label>included_projects</rdfs:label>
    <rdfs:comment>Optional. Names of the projects in scope.
Format: 'projects/{project_number}'</rdfs:comment>
    <rdfs:domain rdf:resource="http://example.org/onto/class/google_os_config_v2_policy_orchestrator_for_organization"/>
    <rdfs:range rdf:resource="http://www.w3.org/2001/XMLSchema#string"/>
  </owl:DatatypeProperty>
  <owl:DatatypeProperty rdf:about="http://example.org/onto/prop/google_os_config_v2_policy_orchestrator_for_organization_create">
    <rdfs:label>create</rdfs:label>
    <rdfs:domain rdf:resource="http://example.org/onto/class/google_os_config_v2_policy_orchestrator_for_organization"/>
    <rdfs:range rdf:resource="http://www.w3.org/2001/XMLSchema#string"/>
  </owl:DatatypeProperty>
  <owl:DatatypeProperty rdf:about="http://example.org/onto/prop/google_os_config_v2_policy_orchestrator_for_organization_delete">
    <rdfs:label>delete</rdfs:label>
    <rdfs:domain rdf:resource="http://example.org/onto/class/google_os_config_v2_policy_orchestrator_for_organization"/>
    <rdfs:range rdf:resource="http://www.w3.org/2001/XMLSchema#string"/>
  </owl:DatatypeProperty>
  <owl:DatatypeProperty rdf:about="http://example.org/onto/prop/google_os_config_v2_policy_orchestrator_for_organization_update">
    <rdfs:label>update</rdfs:label>
    <rdfs:domain rdf:resource="http://example.org/onto/class/google_os_config_v2_policy_orchestrator_for_organization"/>
    <rdfs:range rdf:resource="http://www.w3.org/2001/XMLSchema#string"/>
  </owl:DatatypeProperty>
</rdf:RDF>
