<?xml version="1.0" encoding="UTF-8"?>
<rdf:RDF
  xmlns:rdf="http://www.w3.org/1999/02/22-rdf-syntax-ns#"
  xmlns:rdfs="http://www.w3.org/2000/01/rdf-schema#"
  xmlns:owl="http://www.w3.org/2002/07/owl#"
  xmlns:xsd="http://www.w3.org/2001/XMLSchema#"
  xml:base="http://example.org/onto/">
  <owl:Class rdf:about="http://example.org/onto/class/google_service_account_key">
    <rdfs:label>google_service_account_key</rdfs:label>
  </owl:Class>
  <owl:DatatypeProperty rdf:about="http://example.org/onto/prop/google_service_account_key_id">
    <rdfs:label>id</rdfs:label>
    <rdfs:domain rdf:resource="http://example.org/onto/class/google_service_account_key"/>
    <rdfs:range rdf:resource="http://www.w3.org/2001/XMLSchema#string"/>
  </owl:DatatypeProperty>
  <owl:DatatypeProperty rdf:about="http://example.org/onto/prop/google_service_account_key_keepers">
    <rdfs:label>keepers</rdfs:label>
    <rdfs:comment>Arbitrary map of values that, when changed, will trigger recreation of resource.</rdfs:comment>
    <rdfs:domain rdf:resource="http://example.org/onto/class/google_service_account_key"/>
    <rdfs:range rdf:resource="http://www.w3.org/2001/XMLSchema#string"/>
  </owl:DatatypeProperty>
  <owl:DatatypeProperty rdf:about="http://example.org/onto/prop/google_service_account_key_key_algorithm">
    <rdfs:label>key_algorithm</rdfs:label>
    <rdfs:comment>The algorithm used to generate the key, used only on create. KEY_ALG_RSA_2048 is the default algorithm. Valid values are: "KEY_ALG_RSA_1024", "KEY_ALG_RSA_2048".</rdfs:comment>
    <rdfs:domain rdf:resource="http://example.org/onto/class/google_service_account_key"/>
    <rdfs:range rdf:resource="http://www.w3.org/2001/XMLSchema#string"/>
  </owl:DatatypeProperty>
  <owl:DatatypeProperty rdf:about="http://example.org/onto/prop/google_service_account_key_name">
    <rdfs:label>name</rdfs:label>
    <rdfs:comment>The name used for this key pair</rdfs:comment>
    <rdfs:domain rdf:resource="http://example.org/onto/class/google_service_account_key"/>
    <rdfs:range rdf:resource="http://www.w3.org/2001/XMLSchema#string"/>
  </owl:DatatypeProperty>
  <owl:DatatypeProperty rdf:about="http://example.org/onto/prop/google_service_account_key_private_key">
    <rdfs:label>private_key</rdfs:label>
    <rdfs:comment>The private key in JSON format, base64 encoded. This is what you normally get as a file when creating service account keys through the CLI or web console. This is only populated when creating a new key.</rdfs:comment>
    <rdfs:domain rdf:resource="http://example.org/onto/class/google_service_account_key"/>
    <rdfs:range rdf:resource="http://www.w3.org/2001/XMLSchema#string"/>
  </owl:DatatypeProperty>
  <owl:DatatypeProperty rdf:about="http://example.org/onto/prop/google_service_account_key_private_key_type">
    <rdfs:label>private_key_type</rdfs:label>
    <rdfs:domain rdf:resource="http://example.org/onto/class/google_service_account_key"/>
    <rdfs:range rdf:resource="http://www.w3.org/2001/XMLSchema#string"/>
  </owl:DatatypeProperty>
  <owl:DatatypeProperty rdf:about="http://example.org/onto/prop/google_service_account_key_public_key">
    <rdfs:label>public_key</rdfs:label>
    <rdfs:comment>The public key, base64 encoded</rdfs:comment>
    <rdfs:domain rdf:resource="http://example.org/onto/class/google_service_account_key"/>
    <rdfs:range rdf:resource="http://www.w3.org/2001/XMLSchema#string"/>
  </owl:DatatypeProperty>
  <owl:DatatypeProperty rdf:about="http://example.org/onto/prop/google_service_account_key_public_key_data">
    <rdfs:label>public_key_data</rdfs:label>
    <rdfs:comment>A field that allows clients to upload their own public key. If set, use this public key data to create a service account key for given service account. Please note, the expected format for this field is a base64 encoded X509_PEM.</rdfs:comment>
    <rdfs:domain rdf:resource="http://example.org/onto/class/google_service_account_key"/>
    <rdfs:range rdf:resource="http://www.w3.org/2001/XMLSchema#string"/>
  </owl:DatatypeProperty>
  <owl:DatatypeProperty rdf:about="http://example.org/onto/prop/google_service_account_key_public_key_type">
    <rdfs:label>public_key_type</rdfs:label>
    <rdfs:domain rdf:resource="http://example.org/onto/class/google_service_account_key"/>
    <rdfs:range rdf:resource="http://www.w3.org/2001/XMLSchema#string"/>
  </owl:DatatypeProperty>
  <owl:DatatypeProperty rdf:about="http://example.org/onto/prop/google_service_account_key_service_account_id">
    <rdfs:label>service_account_id</rdfs:label>
    <rdfs:comment>The ID of the parent service account of the key. This can be a string in the format {ACCOUNT} or projects/{PROJECT_ID}/serviceAccounts/{ACCOUNT}, where {ACCOUNT} is the email address or unique id of the service account. If the {ACCOUNT} syntax is used, the project will be inferred from the provider's configuration.</rdfs:comment>
    <rdfs:domain rdf:resource="http://example.org/onto/class/google_service_account_key"/>
    <rdfs:range rdf:resource="http://www.w3.org/2001/XMLSchema#string"/>
  </owl:DatatypeProperty>
  <owl:DatatypeProperty rdf:about="http://example.org/onto/prop/google_service_account_key_valid_after">
    <rdfs:label>valid_after</rdfs:label>
    <rdfs:comment>The key can be used after this timestamp. A timestamp in RFC3339 UTC "Zulu" format, accurate to nanoseconds. Example: "2014-10-02T15:01:23.045123456Z".</rdfs:comment>
    <rdfs:domain rdf:resource="http://example.org/onto/class/google_service_account_key"/>
    <rdfs:range rdf:resource="http://www.w3.org/2001/XMLSchema#string"/>
  </owl:DatatypeProperty>
  <owl:DatatypeProperty rdf:about="http://example.org/onto/prop/google_service_account_key_valid_before">
    <rdfs:label>valid_before</rdfs:label>
    <rdfs:comment>The key can be used before this timestamp. A timestamp in RFC3339 UTC "Zulu" format, accurate to nanoseconds. Example: "2014-10-02T15:01:23.045123456Z".</rdfs:comment>
    <rdfs:domain rdf:resource="http://example.org/onto/class/google_service_account_key"/>
    <rdfs:range rdf:resource="http://www.w3.org/2001/XMLSchema#string"/>
  </owl:DatatypeProperty>
</rdf:RDF>
