<?xml version="1.0" encoding="UTF-8"?>
<rdf:RDF
  xmlns:rdf="http://www.w3.org/1999/02/22-rdf-syntax-ns#"
  xmlns:rdfs="http://www.w3.org/2000/01/rdf-schema#"
  xmlns:owl="http://www.w3.org/2002/07/owl#"
  xmlns:xsd="http://www.w3.org/2001/XMLSchema#"
  xml:base="http://example.org/onto/">
  <owl:Class rdf:about="http://example.org/onto/class/google_compute_security_policy_rule">
    <rdfs:label>google_compute_security_policy_rule</rdfs:label>
    <rdfs:comment>#
#     ***     AUTO GENERATED CODE    ***    Type: MMv1     ***
#
# ----------------------------------------------------------------------------
#
#     This code is generated by Magic Modules using the following:
#
#     Configuration: https:#github.com/GoogleCloudPlatform/magic-modules/tree/main/mmv1/products/compute/SecurityPolicyRule.yaml
#     Template:      https:#github.com/GoogleCloudPlatform/magic-modules/tree/main/mmv1/templates/terraform/resource.html.markdown.tmpl
#
#     DO NOT EDIT this file directly. Any changes made to this file will be
#     overwritten during the next generation cycle.
#
# ----------------------------------------------------------------------------
subcategory: "Compute Engine"
description: |-
  A rule for the SecurityPolicy.
---</rdfs:comment>
  </owl:Class>
  <owl:DatatypeProperty rdf:about="http://example.org/onto/prop/google_compute_security_policy_rule_action">
    <rdfs:label>action</rdfs:label>
    <rdfs:comment>The Action to perform when the rule is matched. The following are the valid actions:

* allow: allow access to target.

* deny(STATUS): deny access to target, returns the HTTP response code specified. Valid values for STATUS are 403, 404, and 502.

* rate_based_ban: limit client traffic to the configured threshold and ban the client if the traffic exceeds the threshold. Configure parameters for this action in RateLimitOptions. Requires rateLimitOptions to be set.

* redirect: redirect to a different target. This can either be an internal reCAPTCHA redirect, or an external URL-based redirect via a 302 response. Parameters for this action can be configured via redirectOptions. This action is only supported in Global Security Policies of type CLOUD_ARMOR.

* throttle: limit client traffic to the configured threshold. Configure parameters for this action in rateLimitOptions. Requires rateLimitOptions to be set for this.</rdfs:comment>
    <rdfs:domain rdf:resource="http://example.org/onto/class/google_compute_security_policy_rule"/>
    <rdfs:range rdf:resource="http://www.w3.org/2001/XMLSchema#string"/>
  </owl:DatatypeProperty>
  <owl:DatatypeProperty rdf:about="http://example.org/onto/prop/google_compute_security_policy_rule_description">
    <rdfs:label>description</rdfs:label>
    <rdfs:comment>An optional description of this resource. Provide this property when you create the resource.</rdfs:comment>
    <rdfs:domain rdf:resource="http://example.org/onto/class/google_compute_security_policy_rule"/>
    <rdfs:range rdf:resource="http://www.w3.org/2001/XMLSchema#string"/>
  </owl:DatatypeProperty>
  <owl:DatatypeProperty rdf:about="http://example.org/onto/prop/google_compute_security_policy_rule_id">
    <rdfs:label>id</rdfs:label>
    <rdfs:domain rdf:resource="http://example.org/onto/class/google_compute_security_policy_rule"/>
    <rdfs:range rdf:resource="http://www.w3.org/2001/XMLSchema#string"/>
  </owl:DatatypeProperty>
  <owl:DatatypeProperty rdf:about="http://example.org/onto/prop/google_compute_security_policy_rule_preview">
    <rdfs:label>preview</rdfs:label>
    <rdfs:comment>If set to true, the specified action is not enforced.</rdfs:comment>
    <rdfs:domain rdf:resource="http://example.org/onto/class/google_compute_security_policy_rule"/>
    <rdfs:range rdf:resource="http://www.w3.org/2001/XMLSchema#string"/>
  </owl:DatatypeProperty>
  <owl:DatatypeProperty rdf:about="http://example.org/onto/prop/google_compute_security_policy_rule_priority">
    <rdfs:label>priority</rdfs:label>
    <rdfs:comment>An integer indicating the priority of a rule in the list.
The priority must be a positive value between 0 and 2147483647.
Rules are evaluated from highest to lowest priority where 0 is the highest priority and 2147483647 is the lowest priority.</rdfs:comment>
    <rdfs:domain rdf:resource="http://example.org/onto/class/google_compute_security_policy_rule"/>
    <rdfs:range rdf:resource="http://www.w3.org/2001/XMLSchema#string"/>
  </owl:DatatypeProperty>
  <owl:DatatypeProperty rdf:about="http://example.org/onto/prop/google_compute_security_policy_rule_project">
    <rdfs:label>project</rdfs:label>
    <rdfs:domain rdf:resource="http://example.org/onto/class/google_compute_security_policy_rule"/>
    <rdfs:range rdf:resource="http://www.w3.org/2001/XMLSchema#string"/>
  </owl:DatatypeProperty>
  <owl:DatatypeProperty rdf:about="http://example.org/onto/prop/google_compute_security_policy_rule_security_policy">
    <rdfs:label>security_policy</rdfs:label>
    <rdfs:comment>The name of the security policy this rule belongs to.</rdfs:comment>
    <rdfs:domain rdf:resource="http://example.org/onto/class/google_compute_security_policy_rule"/>
    <rdfs:range rdf:resource="http://www.w3.org/2001/XMLSchema#string"/>
  </owl:DatatypeProperty>
  <owl:DatatypeProperty rdf:about="http://example.org/onto/prop/google_compute_security_policy_rule_header_name">
    <rdfs:label>header_name</rdfs:label>
    <rdfs:comment>The name of the header to set.</rdfs:comment>
    <rdfs:domain rdf:resource="http://example.org/onto/class/google_compute_security_policy_rule"/>
    <rdfs:range rdf:resource="http://www.w3.org/2001/XMLSchema#string"/>
  </owl:DatatypeProperty>
  <owl:DatatypeProperty rdf:about="http://example.org/onto/prop/google_compute_security_policy_rule_header_value">
    <rdfs:label>header_value</rdfs:label>
    <rdfs:comment>The value to set the named header to.</rdfs:comment>
    <rdfs:domain rdf:resource="http://example.org/onto/class/google_compute_security_policy_rule"/>
    <rdfs:range rdf:resource="http://www.w3.org/2001/XMLSchema#string"/>
  </owl:DatatypeProperty>
  <owl:DatatypeProperty rdf:about="http://example.org/onto/prop/google_compute_security_policy_rule_versioned_expr">
    <rdfs:label>versioned_expr</rdfs:label>
    <rdfs:comment>Preconfigured versioned expression. If this field is specified, config must also be specified.
Available preconfigured expressions along with their requirements are: SRC_IPS_V1 - must specify the corresponding srcIpRange field in config. Possible values: ["SRC_IPS_V1"]</rdfs:comment>
    <rdfs:domain rdf:resource="http://example.org/onto/class/google_compute_security_policy_rule"/>
    <rdfs:range rdf:resource="http://www.w3.org/2001/XMLSchema#string"/>
  </owl:DatatypeProperty>
  <owl:DatatypeProperty rdf:about="http://example.org/onto/prop/google_compute_security_policy_rule_src_ip_ranges">
    <rdfs:label>src_ip_ranges</rdfs:label>
    <rdfs:comment>CIDR IP address range. Maximum number of srcIpRanges allowed is 10.</rdfs:comment>
    <rdfs:domain rdf:resource="http://example.org/onto/class/google_compute_security_policy_rule"/>
    <rdfs:range rdf:resource="http://www.w3.org/2001/XMLSchema#string"/>
  </owl:DatatypeProperty>
  <owl:DatatypeProperty rdf:about="http://example.org/onto/prop/google_compute_security_policy_rule_expression">
    <rdfs:label>expression</rdfs:label>
    <rdfs:comment>Textual representation of an expression in Common Expression Language syntax. The application context of the containing message determines which well-known feature set of CEL is supported.</rdfs:comment>
    <rdfs:domain rdf:resource="http://example.org/onto/class/google_compute_security_policy_rule"/>
    <rdfs:range rdf:resource="http://www.w3.org/2001/XMLSchema#string"/>
  </owl:DatatypeProperty>
  <owl:DatatypeProperty rdf:about="http://example.org/onto/prop/google_compute_security_policy_rule_action_token_site_keys">
    <rdfs:label>action_token_site_keys</rdfs:label>
    <rdfs:comment>A list of site keys to be used during the validation of reCAPTCHA action-tokens. The provided site keys need to be created from reCAPTCHA API under the same project where the security policy is created.</rdfs:comment>
    <rdfs:domain rdf:resource="http://example.org/onto/class/google_compute_security_policy_rule"/>
    <rdfs:range rdf:resource="http://www.w3.org/2001/XMLSchema#string"/>
  </owl:DatatypeProperty>
  <owl:DatatypeProperty rdf:about="http://example.org/onto/prop/google_compute_security_policy_rule_session_token_site_keys">
    <rdfs:label>session_token_site_keys</rdfs:label>
    <rdfs:comment>A list of site keys to be used during the validation of reCAPTCHA session-tokens. The provided site keys need to be created from reCAPTCHA API under the same project where the security policy is created.</rdfs:comment>
    <rdfs:domain rdf:resource="http://example.org/onto/class/google_compute_security_policy_rule"/>
    <rdfs:range rdf:resource="http://www.w3.org/2001/XMLSchema#string"/>
  </owl:DatatypeProperty>
  <owl:DatatypeProperty rdf:about="http://example.org/onto/prop/google_compute_security_policy_rule_target_rule_ids">
    <rdfs:label>target_rule_ids</rdfs:label>
    <rdfs:comment>A list of target rule IDs under the WAF rule set to apply the preconfigured WAF exclusion.
If omitted, it refers to all the rule IDs under the WAF rule set.</rdfs:comment>
    <rdfs:domain rdf:resource="http://example.org/onto/class/google_compute_security_policy_rule"/>
    <rdfs:range rdf:resource="http://www.w3.org/2001/XMLSchema#string"/>
  </owl:DatatypeProperty>
  <owl:DatatypeProperty rdf:about="http://example.org/onto/prop/google_compute_security_policy_rule_target_rule_set">
    <rdfs:label>target_rule_set</rdfs:label>
    <rdfs:comment>Target WAF rule set to apply the preconfigured WAF exclusion.</rdfs:comment>
    <rdfs:domain rdf:resource="http://example.org/onto/class/google_compute_security_policy_rule"/>
    <rdfs:range rdf:resource="http://www.w3.org/2001/XMLSchema#string"/>
  </owl:DatatypeProperty>
  <owl:DatatypeProperty rdf:about="http://example.org/onto/prop/google_compute_security_policy_rule_operator">
    <rdfs:label>operator</rdfs:label>
    <rdfs:comment>You can specify an exact match or a partial match by using a field operator and a field value.
Available options:
EQUALS: The operator matches if the field value equals the specified value.
STARTS_WITH: The operator matches if the field value starts with the specified value.
ENDS_WITH: The operator matches if the field value ends with the specified value.
CONTAINS: The operator matches if the field value contains the specified value.
EQUALS_ANY: The operator matches if the field value is any value.</rdfs:comment>
    <rdfs:domain rdf:resource="http://example.org/onto/class/google_compute_security_policy_rule"/>
    <rdfs:range rdf:resource="http://www.w3.org/2001/XMLSchema#string"/>
  </owl:DatatypeProperty>
  <owl:DatatypeProperty rdf:about="http://example.org/onto/prop/google_compute_security_policy_rule_value">
    <rdfs:label>value</rdfs:label>
    <rdfs:comment>A request field matching the specified value will be excluded from inspection during preconfigured WAF evaluation.
The field value must be given if the field operator is not EQUALS_ANY, and cannot be given if the field operator is EQUALS_ANY.</rdfs:comment>
    <rdfs:domain rdf:resource="http://example.org/onto/class/google_compute_security_policy_rule"/>
    <rdfs:range rdf:resource="http://www.w3.org/2001/XMLSchema#string"/>
  </owl:DatatypeProperty>
  <owl:DatatypeProperty rdf:about="http://example.org/onto/prop/google_compute_security_policy_rule_operator">
    <rdfs:label>operator</rdfs:label>
    <rdfs:comment>You can specify an exact match or a partial match by using a field operator and a field value.
Available options:
EQUALS: The operator matches if the field value equals the specified value.
STARTS_WITH: The operator matches if the field value starts with the specified value.
ENDS_WITH: The operator matches if the field value ends with the specified value.
CONTAINS: The operator matches if the field value contains the specified value.
EQUALS_ANY: The operator matches if the field value is any value.</rdfs:comment>
    <rdfs:domain rdf:resource="http://example.org/onto/class/google_compute_security_policy_rule"/>
    <rdfs:range rdf:resource="http://www.w3.org/2001/XMLSchema#string"/>
  </owl:DatatypeProperty>
  <owl:DatatypeProperty rdf:about="http://example.org/onto/prop/google_compute_security_policy_rule_value">
    <rdfs:label>value</rdfs:label>
    <rdfs:comment>A request field matching the specified value will be excluded from inspection during preconfigured WAF evaluation.
The field value must be given if the field operator is not EQUALS_ANY, and cannot be given if the field operator is EQUALS_ANY.</rdfs:comment>
    <rdfs:domain rdf:resource="http://example.org/onto/class/google_compute_security_policy_rule"/>
    <rdfs:range rdf:resource="http://www.w3.org/2001/XMLSchema#string"/>
  </owl:DatatypeProperty>
  <owl:DatatypeProperty rdf:about="http://example.org/onto/prop/google_compute_security_policy_rule_operator">
    <rdfs:label>operator</rdfs:label>
    <rdfs:comment>You can specify an exact match or a partial match by using a field operator and a field value.
Available options:
EQUALS: The operator matches if the field value equals the specified value.
STARTS_WITH: The operator matches if the field value starts with the specified value.
ENDS_WITH: The operator matches if the field value ends with the specified value.
CONTAINS: The operator matches if the field value contains the specified value.
EQUALS_ANY: The operator matches if the field value is any value.</rdfs:comment>
    <rdfs:domain rdf:resource="http://example.org/onto/class/google_compute_security_policy_rule"/>
    <rdfs:range rdf:resource="http://www.w3.org/2001/XMLSchema#string"/>
  </owl:DatatypeProperty>
  <owl:DatatypeProperty rdf:about="http://example.org/onto/prop/google_compute_security_policy_rule_value">
    <rdfs:label>value</rdfs:label>
    <rdfs:comment>A request field matching the specified value will be excluded from inspection during preconfigured WAF evaluation.
The field value must be given if the field operator is not EQUALS_ANY, and cannot be given if the field operator is EQUALS_ANY.</rdfs:comment>
    <rdfs:domain rdf:resource="http://example.org/onto/class/google_compute_security_policy_rule"/>
    <rdfs:range rdf:resource="http://www.w3.org/2001/XMLSchema#string"/>
  </owl:DatatypeProperty>
  <owl:DatatypeProperty rdf:about="http://example.org/onto/prop/google_compute_security_policy_rule_operator">
    <rdfs:label>operator</rdfs:label>
    <rdfs:comment>You can specify an exact match or a partial match by using a field operator and a field value.
Available options:
EQUALS: The operator matches if the field value equals the specified value.
STARTS_WITH: The operator matches if the field value starts with the specified value.
ENDS_WITH: The operator matches if the field value ends with the specified value.
CONTAINS: The operator matches if the field value contains the specified value.
EQUALS_ANY: The operator matches if the field value is any value.</rdfs:comment>
    <rdfs:domain rdf:resource="http://example.org/onto/class/google_compute_security_policy_rule"/>
    <rdfs:range rdf:resource="http://www.w3.org/2001/XMLSchema#string"/>
  </owl:DatatypeProperty>
  <owl:DatatypeProperty rdf:about="http://example.org/onto/prop/google_compute_security_policy_rule_value">
    <rdfs:label>value</rdfs:label>
    <rdfs:comment>A request field matching the specified value will be excluded from inspection during preconfigured WAF evaluation.
The field value must be given if the field operator is not EQUALS_ANY, and cannot be given if the field operator is EQUALS_ANY.</rdfs:comment>
    <rdfs:domain rdf:resource="http://example.org/onto/class/google_compute_security_policy_rule"/>
    <rdfs:range rdf:resource="http://www.w3.org/2001/XMLSchema#string"/>
  </owl:DatatypeProperty>
  <owl:DatatypeProperty rdf:about="http://example.org/onto/prop/google_compute_security_policy_rule_ban_duration_sec">
    <rdfs:label>ban_duration_sec</rdfs:label>
    <rdfs:comment>Can only be specified if the action for the rule is "rate_based_ban".
If specified, determines the time (in seconds) the traffic will continue to be banned by the rate limit after the rate falls below the threshold.</rdfs:comment>
    <rdfs:domain rdf:resource="http://example.org/onto/class/google_compute_security_policy_rule"/>
    <rdfs:range rdf:resource="http://www.w3.org/2001/XMLSchema#string"/>
  </owl:DatatypeProperty>
  <owl:DatatypeProperty rdf:about="http://example.org/onto/prop/google_compute_security_policy_rule_conform_action">
    <rdfs:label>conform_action</rdfs:label>
    <rdfs:comment>Action to take for requests that are under the configured rate limit threshold.
Valid option is "allow" only.</rdfs:comment>
    <rdfs:domain rdf:resource="http://example.org/onto/class/google_compute_security_policy_rule"/>
    <rdfs:range rdf:resource="http://www.w3.org/2001/XMLSchema#string"/>
  </owl:DatatypeProperty>
  <owl:DatatypeProperty rdf:about="http://example.org/onto/prop/google_compute_security_policy_rule_enforce_on_key">
    <rdfs:label>enforce_on_key</rdfs:label>
    <rdfs:comment>Determines the key to enforce the rateLimitThreshold on. Possible values are:
* ALL: A single rate limit threshold is applied to all the requests matching this rule. This is the default value if "enforceOnKey" is not configured.
* IP: The source IP address of the request is the key. Each IP has this limit enforced separately.
* HTTP_HEADER: The value of the HTTP header whose name is configured under "enforceOnKeyName". The key value is truncated to the first 128 bytes of the header value. If no such header is present in the request, the key type defaults to ALL.
* XFF_IP: The first IP address (i.e. the originating client IP address) specified in the list of IPs under X-Forwarded-For HTTP header. If no such header is present or the value is not a valid IP, the key defaults to the source IP address of the request i.e. key type IP.
* HTTP_COOKIE: The value of the HTTP cookie whose name is configured under "enforceOnKeyName". The key value is truncated to the first 128 bytes of the cookie value. If no such cookie is present in the request, the key type defaults to ALL.
* HTTP_PATH: The URL path of the HTTP request. The key value is truncated to the first 128 bytes.
* SNI: Server name indication in the TLS session of the HTTPS request. The key value is truncated to the first 128 bytes. The key type defaults to ALL on a HTTP session.
* REGION_CODE: The country/region from which the request originates.
* TLS_JA3_FINGERPRINT: JA3 TLS/SSL fingerprint if the client connects using HTTPS, HTTP/2 or HTTP/3. If not available, the key type defaults to ALL.
* TLS_JA4_FINGERPRINT: JA4 TLS/SSL fingerprint if the client connects using HTTPS, HTTP/2 or HTTP/3. If not available, the key type defaults to ALL.
* USER_IP: The IP address of the originating client, which is resolved based on "userIpRequestHeaders" configured with the security policy. If there is no "userIpRequestHeaders" configuration or an IP address cannot be resolved from it, the key type defaults to IP. Possible values: ["ALL", "IP", "HTTP_HEADER", "XFF_IP", "HTTP_COOKIE", "HTTP_PATH", "SNI", "REGION_CODE", "TLS_JA3_FINGERPRINT", "TLS_JA4_FINGERPRINT", "USER_IP"]</rdfs:comment>
    <rdfs:domain rdf:resource="http://example.org/onto/class/google_compute_security_policy_rule"/>
    <rdfs:range rdf:resource="http://www.w3.org/2001/XMLSchema#string"/>
  </owl:DatatypeProperty>
  <owl:DatatypeProperty rdf:about="http://example.org/onto/prop/google_compute_security_policy_rule_enforce_on_key_name">
    <rdfs:label>enforce_on_key_name</rdfs:label>
    <rdfs:comment>Rate limit key name applicable only for the following key types:
HTTP_HEADER -- Name of the HTTP header whose value is taken as the key value.
HTTP_COOKIE -- Name of the HTTP cookie whose value is taken as the key value.</rdfs:comment>
    <rdfs:domain rdf:resource="http://example.org/onto/class/google_compute_security_policy_rule"/>
    <rdfs:range rdf:resource="http://www.w3.org/2001/XMLSchema#string"/>
  </owl:DatatypeProperty>
  <owl:DatatypeProperty rdf:about="http://example.org/onto/prop/google_compute_security_policy_rule_exceed_action">
    <rdfs:label>exceed_action</rdfs:label>
    <rdfs:comment>Action to take for requests that are above the configured rate limit threshold, to either deny with a specified HTTP response code, or redirect to a different endpoint.
Valid options are deny(STATUS), where valid values for STATUS are 403, 404, 429, and 502.</rdfs:comment>
    <rdfs:domain rdf:resource="http://example.org/onto/class/google_compute_security_policy_rule"/>
    <rdfs:range rdf:resource="http://www.w3.org/2001/XMLSchema#string"/>
  </owl:DatatypeProperty>
  <owl:DatatypeProperty rdf:about="http://example.org/onto/prop/google_compute_security_policy_rule_count">
    <rdfs:label>count</rdfs:label>
    <rdfs:comment>Number of HTTP(S) requests for calculating the threshold.</rdfs:comment>
    <rdfs:domain rdf:resource="http://example.org/onto/class/google_compute_security_policy_rule"/>
    <rdfs:range rdf:resource="http://www.w3.org/2001/XMLSchema#string"/>
  </owl:DatatypeProperty>
  <owl:DatatypeProperty rdf:about="http://example.org/onto/prop/google_compute_security_policy_rule_interval_sec">
    <rdfs:label>interval_sec</rdfs:label>
    <rdfs:comment>Interval over which the threshold is computed.</rdfs:comment>
    <rdfs:domain rdf:resource="http://example.org/onto/class/google_compute_security_policy_rule"/>
    <rdfs:range rdf:resource="http://www.w3.org/2001/XMLSchema#string"/>
  </owl:DatatypeProperty>
  <owl:DatatypeProperty rdf:about="http://example.org/onto/prop/google_compute_security_policy_rule_enforce_on_key_name">
    <rdfs:label>enforce_on_key_name</rdfs:label>
    <rdfs:comment>Rate limit key name applicable only for the following key types:
HTTP_HEADER -- Name of the HTTP header whose value is taken as the key value.
HTTP_COOKIE -- Name of the HTTP cookie whose value is taken as the key value.</rdfs:comment>
    <rdfs:domain rdf:resource="http://example.org/onto/class/google_compute_security_policy_rule"/>
    <rdfs:range rdf:resource="http://www.w3.org/2001/XMLSchema#string"/>
  </owl:DatatypeProperty>
  <owl:DatatypeProperty rdf:about="http://example.org/onto/prop/google_compute_security_policy_rule_enforce_on_key_type">
    <rdfs:label>enforce_on_key_type</rdfs:label>
    <rdfs:comment>Determines the key to enforce the rateLimitThreshold on. Possible values are:
* ALL: A single rate limit threshold is applied to all the requests matching this rule. This is the default value if "enforceOnKeyConfigs" is not configured.
* IP: The source IP address of the request is the key. Each IP has this limit enforced separately.
* HTTP_HEADER: The value of the HTTP header whose name is configured under "enforceOnKeyName". The key value is truncated to the first 128 bytes of the header value. If no such header is present in the request, the key type defaults to ALL.
* XFF_IP: The first IP address (i.e. the originating client IP address) specified in the list of IPs under X-Forwarded-For HTTP header. If no such header is present or the value is not a valid IP, the key defaults to the source IP address of the request i.e. key type IP.
* HTTP_COOKIE: The value of the HTTP cookie whose name is configured under "enforceOnKeyName". The key value is truncated to the first 128 bytes of the cookie value. If no such cookie is present in the request, the key type defaults to ALL.
* HTTP_PATH: The URL path of the HTTP request. The key value is truncated to the first 128 bytes.
* SNI: Server name indication in the TLS session of the HTTPS request. The key value is truncated to the first 128 bytes. The key type defaults to ALL on a HTTP session.
* REGION_CODE: The country/region from which the request originates.
* TLS_JA3_FINGERPRINT: JA3 TLS/SSL fingerprint if the client connects using HTTPS, HTTP/2 or HTTP/3. If not available, the key type defaults to ALL.
* TLS_JA4_FINGERPRINT: JA4 TLS/SSL fingerprint if the client connects using HTTPS, HTTP/2 or HTTP/3. If not available, the key type defaults to ALL.
* USER_IP: The IP address of the originating client, which is resolved based on "userIpRequestHeaders" configured with the security policy. If there is no "userIpRequestHeaders" configuration or an IP address cannot be resolved from it, the key type defaults to IP. Possible values: ["ALL", "IP", "HTTP_HEADER", "XFF_IP", "HTTP_COOKIE", "HTTP_PATH", "SNI", "REGION_CODE", "TLS_JA3_FINGERPRINT", "TLS_JA4_FINGERPRINT", "USER_IP"]</rdfs:comment>
    <rdfs:domain rdf:resource="http://example.org/onto/class/google_compute_security_policy_rule"/>
    <rdfs:range rdf:resource="http://www.w3.org/2001/XMLSchema#string"/>
  </owl:DatatypeProperty>
  <owl:DatatypeProperty rdf:about="http://example.org/onto/prop/google_compute_security_policy_rule_target">
    <rdfs:label>target</rdfs:label>
    <rdfs:comment>Target for the redirect action. This is required if the type is EXTERNAL_302 and cannot be specified for GOOGLE_RECAPTCHA.</rdfs:comment>
    <rdfs:domain rdf:resource="http://example.org/onto/class/google_compute_security_policy_rule"/>
    <rdfs:range rdf:resource="http://www.w3.org/2001/XMLSchema#string"/>
  </owl:DatatypeProperty>
  <owl:DatatypeProperty rdf:about="http://example.org/onto/prop/google_compute_security_policy_rule_type">
    <rdfs:label>type</rdfs:label>
    <rdfs:comment>Type of the redirect action.</rdfs:comment>
    <rdfs:domain rdf:resource="http://example.org/onto/class/google_compute_security_policy_rule"/>
    <rdfs:range rdf:resource="http://www.w3.org/2001/XMLSchema#string"/>
  </owl:DatatypeProperty>
  <owl:DatatypeProperty rdf:about="http://example.org/onto/prop/google_compute_security_policy_rule_count">
    <rdfs:label>count</rdfs:label>
    <rdfs:comment>Number of HTTP(S) requests for calculating the threshold.</rdfs:comment>
    <rdfs:domain rdf:resource="http://example.org/onto/class/google_compute_security_policy_rule"/>
    <rdfs:range rdf:resource="http://www.w3.org/2001/XMLSchema#string"/>
  </owl:DatatypeProperty>
  <owl:DatatypeProperty rdf:about="http://example.org/onto/prop/google_compute_security_policy_rule_interval_sec">
    <rdfs:label>interval_sec</rdfs:label>
    <rdfs:comment>Interval over which the threshold is computed.</rdfs:comment>
    <rdfs:domain rdf:resource="http://example.org/onto/class/google_compute_security_policy_rule"/>
    <rdfs:range rdf:resource="http://www.w3.org/2001/XMLSchema#string"/>
  </owl:DatatypeProperty>
  <owl:DatatypeProperty rdf:about="http://example.org/onto/prop/google_compute_security_policy_rule_target">
    <rdfs:label>target</rdfs:label>
    <rdfs:comment>Target for the redirect action. This is required if the type is EXTERNAL_302 and cannot be specified for GOOGLE_RECAPTCHA.</rdfs:comment>
    <rdfs:domain rdf:resource="http://example.org/onto/class/google_compute_security_policy_rule"/>
    <rdfs:range rdf:resource="http://www.w3.org/2001/XMLSchema#string"/>
  </owl:DatatypeProperty>
  <owl:DatatypeProperty rdf:about="http://example.org/onto/prop/google_compute_security_policy_rule_type">
    <rdfs:label>type</rdfs:label>
    <rdfs:comment>Type of the redirect action.</rdfs:comment>
    <rdfs:domain rdf:resource="http://example.org/onto/class/google_compute_security_policy_rule"/>
    <rdfs:range rdf:resource="http://www.w3.org/2001/XMLSchema#string"/>
  </owl:DatatypeProperty>
  <owl:DatatypeProperty rdf:about="http://example.org/onto/prop/google_compute_security_policy_rule_create">
    <rdfs:label>create</rdfs:label>
    <rdfs:domain rdf:resource="http://example.org/onto/class/google_compute_security_policy_rule"/>
    <rdfs:range rdf:resource="http://www.w3.org/2001/XMLSchema#string"/>
  </owl:DatatypeProperty>
  <owl:DatatypeProperty rdf:about="http://example.org/onto/prop/google_compute_security_policy_rule_delete">
    <rdfs:label>delete</rdfs:label>
    <rdfs:domain rdf:resource="http://example.org/onto/class/google_compute_security_policy_rule"/>
    <rdfs:range rdf:resource="http://www.w3.org/2001/XMLSchema#string"/>
  </owl:DatatypeProperty>
  <owl:DatatypeProperty rdf:about="http://example.org/onto/prop/google_compute_security_policy_rule_update">
    <rdfs:label>update</rdfs:label>
    <rdfs:domain rdf:resource="http://example.org/onto/class/google_compute_security_policy_rule"/>
    <rdfs:range rdf:resource="http://www.w3.org/2001/XMLSchema#string"/>
  </owl:DatatypeProperty>
</rdf:RDF>
