<?xml version="1.0" encoding="UTF-8"?>
<rdf:RDF
  xmlns:rdf="http://www.w3.org/1999/02/22-rdf-syntax-ns#"
  xmlns:rdfs="http://www.w3.org/2000/01/rdf-schema#"
  xmlns:owl="http://www.w3.org/2002/07/owl#"
  xmlns:xsd="http://www.w3.org/2001/XMLSchema#"
  xml:base="http://example.org/onto/">
  <owl:Class rdf:about="http://example.org/onto/class/google_bigquery_analytics_hub_listing">
    <rdfs:label>google_bigquery_analytics_hub_listing</rdfs:label>
    <rdfs:comment>#
#     ***     AUTO GENERATED CODE    ***    Type: MMv1     ***
#
# ----------------------------------------------------------------------------
#
#     This code is generated by Magic Modules using the following:
#
#     Configuration: https:#github.com/GoogleCloudPlatform/magic-modules/tree/main/mmv1/products/bigqueryanalyticshub/Listing.yaml
#     Template:      https:#github.com/GoogleCloudPlatform/magic-modules/tree/main/mmv1/templates/terraform/resource.html.markdown.tmpl
#
#     DO NOT EDIT this file directly. Any changes made to this file will be
#     overwritten during the next generation cycle.
#
# ----------------------------------------------------------------------------
subcategory: "BigQuery Analytics Hub"
description: |-
  A Bigquery Analytics Hub data exchange listing
---</rdfs:comment>
  </owl:Class>
  <owl:DatatypeProperty rdf:about="http://example.org/onto/prop/google_bigquery_analytics_hub_listing_allow_only_metadata_sharing">
    <rdfs:label>allow_only_metadata_sharing</rdfs:label>
    <rdfs:comment>If true, the listing is only available to get the resource metadata. Listing is non subscribable.</rdfs:comment>
    <rdfs:domain rdf:resource="http://example.org/onto/class/google_bigquery_analytics_hub_listing"/>
    <rdfs:range rdf:resource="http://www.w3.org/2001/XMLSchema#string"/>
  </owl:DatatypeProperty>
  <owl:DatatypeProperty rdf:about="http://example.org/onto/prop/google_bigquery_analytics_hub_listing_categories">
    <rdfs:label>categories</rdfs:label>
    <rdfs:comment>Categories of the listing. Up to two categories are allowed.</rdfs:comment>
    <rdfs:domain rdf:resource="http://example.org/onto/class/google_bigquery_analytics_hub_listing"/>
    <rdfs:range rdf:resource="http://www.w3.org/2001/XMLSchema#string"/>
  </owl:DatatypeProperty>
  <owl:DatatypeProperty rdf:about="http://example.org/onto/prop/google_bigquery_analytics_hub_listing_commercial_info">
    <rdfs:label>commercial_info</rdfs:label>
    <rdfs:comment>Commercial info contains the information about the commercial data products associated with the listing.</rdfs:comment>
    <rdfs:domain rdf:resource="http://example.org/onto/class/google_bigquery_analytics_hub_listing"/>
    <rdfs:range rdf:resource="http://www.w3.org/2001/XMLSchema#string"/>
  </owl:DatatypeProperty>
  <owl:DatatypeProperty rdf:about="http://example.org/onto/prop/google_bigquery_analytics_hub_listing_data_exchange_id">
    <rdfs:label>data_exchange_id</rdfs:label>
    <rdfs:comment>The ID of the data exchange. Must contain only Unicode letters, numbers (0-9), underscores (_). Should not use characters that require URL-escaping, or characters outside of ASCII, spaces.</rdfs:comment>
    <rdfs:domain rdf:resource="http://example.org/onto/class/google_bigquery_analytics_hub_listing"/>
    <rdfs:range rdf:resource="http://www.w3.org/2001/XMLSchema#string"/>
  </owl:DatatypeProperty>
  <owl:DatatypeProperty rdf:about="http://example.org/onto/prop/google_bigquery_analytics_hub_listing_delete_commercial">
    <rdfs:label>delete_commercial</rdfs:label>
    <rdfs:comment>If the listing is commercial then this field must be set to true, otherwise a failure is thrown. This acts as a safety guard to avoid deleting commercial listings accidentally.</rdfs:comment>
    <rdfs:domain rdf:resource="http://example.org/onto/class/google_bigquery_analytics_hub_listing"/>
    <rdfs:range rdf:resource="http://www.w3.org/2001/XMLSchema#string"/>
  </owl:DatatypeProperty>
  <owl:DatatypeProperty rdf:about="http://example.org/onto/prop/google_bigquery_analytics_hub_listing_description">
    <rdfs:label>description</rdfs:label>
    <rdfs:comment>Short description of the listing. The description must not contain Unicode non-characters and C0 and C1 control codes except tabs (HT), new lines (LF), carriage returns (CR), and page breaks (FF).</rdfs:comment>
    <rdfs:domain rdf:resource="http://example.org/onto/class/google_bigquery_analytics_hub_listing"/>
    <rdfs:range rdf:resource="http://www.w3.org/2001/XMLSchema#string"/>
  </owl:DatatypeProperty>
  <owl:DatatypeProperty rdf:about="http://example.org/onto/prop/google_bigquery_analytics_hub_listing_discovery_type">
    <rdfs:label>discovery_type</rdfs:label>
    <rdfs:comment>Specifies the type of discovery on the discovery page. Cannot be set for a restricted listing. Note that this does not control the visibility of the exchange/listing which is defined by IAM permission. Possible values: ["DISCOVERY_TYPE_PRIVATE", "DISCOVERY_TYPE_PUBLIC"]</rdfs:comment>
    <rdfs:domain rdf:resource="http://example.org/onto/class/google_bigquery_analytics_hub_listing"/>
    <rdfs:range rdf:resource="http://www.w3.org/2001/XMLSchema#string"/>
  </owl:DatatypeProperty>
  <owl:DatatypeProperty rdf:about="http://example.org/onto/prop/google_bigquery_analytics_hub_listing_display_name">
    <rdfs:label>display_name</rdfs:label>
    <rdfs:comment>Human-readable display name of the listing. The display name must contain only Unicode letters, numbers (0-9), underscores (_), dashes (-), spaces ( ), ampersands (&) and can't start or end with spaces.</rdfs:comment>
    <rdfs:domain rdf:resource="http://example.org/onto/class/google_bigquery_analytics_hub_listing"/>
    <rdfs:range rdf:resource="http://www.w3.org/2001/XMLSchema#string"/>
  </owl:DatatypeProperty>
  <owl:DatatypeProperty rdf:about="http://example.org/onto/prop/google_bigquery_analytics_hub_listing_documentation">
    <rdfs:label>documentation</rdfs:label>
    <rdfs:comment>Documentation describing the listing.</rdfs:comment>
    <rdfs:domain rdf:resource="http://example.org/onto/class/google_bigquery_analytics_hub_listing"/>
    <rdfs:range rdf:resource="http://www.w3.org/2001/XMLSchema#string"/>
  </owl:DatatypeProperty>
  <owl:DatatypeProperty rdf:about="http://example.org/onto/prop/google_bigquery_analytics_hub_listing_icon">
    <rdfs:label>icon</rdfs:label>
    <rdfs:comment>Base64 encoded image representing the listing.</rdfs:comment>
    <rdfs:domain rdf:resource="http://example.org/onto/class/google_bigquery_analytics_hub_listing"/>
    <rdfs:range rdf:resource="http://www.w3.org/2001/XMLSchema#string"/>
  </owl:DatatypeProperty>
  <owl:DatatypeProperty rdf:about="http://example.org/onto/prop/google_bigquery_analytics_hub_listing_id">
    <rdfs:label>id</rdfs:label>
    <rdfs:domain rdf:resource="http://example.org/onto/class/google_bigquery_analytics_hub_listing"/>
    <rdfs:range rdf:resource="http://www.w3.org/2001/XMLSchema#string"/>
  </owl:DatatypeProperty>
  <owl:DatatypeProperty rdf:about="http://example.org/onto/prop/google_bigquery_analytics_hub_listing_listing_id">
    <rdfs:label>listing_id</rdfs:label>
    <rdfs:comment>The ID of the listing. Must contain only Unicode letters, numbers (0-9), underscores (_). Should not use characters that require URL-escaping, or characters outside of ASCII, spaces.</rdfs:comment>
    <rdfs:domain rdf:resource="http://example.org/onto/class/google_bigquery_analytics_hub_listing"/>
    <rdfs:range rdf:resource="http://www.w3.org/2001/XMLSchema#string"/>
  </owl:DatatypeProperty>
  <owl:DatatypeProperty rdf:about="http://example.org/onto/prop/google_bigquery_analytics_hub_listing_location">
    <rdfs:label>location</rdfs:label>
    <rdfs:comment>The name of the location this data exchange listing.</rdfs:comment>
    <rdfs:domain rdf:resource="http://example.org/onto/class/google_bigquery_analytics_hub_listing"/>
    <rdfs:range rdf:resource="http://www.w3.org/2001/XMLSchema#string"/>
  </owl:DatatypeProperty>
  <owl:DatatypeProperty rdf:about="http://example.org/onto/prop/google_bigquery_analytics_hub_listing_log_linked_dataset_query_user_email">
    <rdfs:label>log_linked_dataset_query_user_email</rdfs:label>
    <rdfs:comment>If true, subscriber email logging is enabled and all queries on the linked dataset will log the email address of the querying user. Once enabled, this setting cannot be turned off.</rdfs:comment>
    <rdfs:domain rdf:resource="http://example.org/onto/class/google_bigquery_analytics_hub_listing"/>
    <rdfs:range rdf:resource="http://www.w3.org/2001/XMLSchema#string"/>
  </owl:DatatypeProperty>
  <owl:DatatypeProperty rdf:about="http://example.org/onto/prop/google_bigquery_analytics_hub_listing_name">
    <rdfs:label>name</rdfs:label>
    <rdfs:comment>The resource name of the listing. e.g. "projects/myproject/locations/US/dataExchanges/123/listings/456"</rdfs:comment>
    <rdfs:domain rdf:resource="http://example.org/onto/class/google_bigquery_analytics_hub_listing"/>
    <rdfs:range rdf:resource="http://www.w3.org/2001/XMLSchema#string"/>
  </owl:DatatypeProperty>
  <owl:DatatypeProperty rdf:about="http://example.org/onto/prop/google_bigquery_analytics_hub_listing_primary_contact">
    <rdfs:label>primary_contact</rdfs:label>
    <rdfs:comment>Email or URL of the primary point of contact of the listing.</rdfs:comment>
    <rdfs:domain rdf:resource="http://example.org/onto/class/google_bigquery_analytics_hub_listing"/>
    <rdfs:range rdf:resource="http://www.w3.org/2001/XMLSchema#string"/>
  </owl:DatatypeProperty>
  <owl:DatatypeProperty rdf:about="http://example.org/onto/prop/google_bigquery_analytics_hub_listing_project">
    <rdfs:label>project</rdfs:label>
    <rdfs:domain rdf:resource="http://example.org/onto/class/google_bigquery_analytics_hub_listing"/>
    <rdfs:range rdf:resource="http://www.w3.org/2001/XMLSchema#string"/>
  </owl:DatatypeProperty>
  <owl:DatatypeProperty rdf:about="http://example.org/onto/prop/google_bigquery_analytics_hub_listing_request_access">
    <rdfs:label>request_access</rdfs:label>
    <rdfs:comment>Email or URL of the request access of the listing. Subscribers can use this reference to request access.</rdfs:comment>
    <rdfs:domain rdf:resource="http://example.org/onto/class/google_bigquery_analytics_hub_listing"/>
    <rdfs:range rdf:resource="http://www.w3.org/2001/XMLSchema#string"/>
  </owl:DatatypeProperty>
  <owl:DatatypeProperty rdf:about="http://example.org/onto/prop/google_bigquery_analytics_hub_listing_state">
    <rdfs:label>state</rdfs:label>
    <rdfs:comment>Current state of the listing.</rdfs:comment>
    <rdfs:domain rdf:resource="http://example.org/onto/class/google_bigquery_analytics_hub_listing"/>
    <rdfs:range rdf:resource="http://www.w3.org/2001/XMLSchema#string"/>
  </owl:DatatypeProperty>
  <owl:DatatypeProperty rdf:about="http://example.org/onto/prop/google_bigquery_analytics_hub_listing_dataset">
    <rdfs:label>dataset</rdfs:label>
    <rdfs:comment>Resource name of the dataset source for this listing. e.g. projects/myproject/datasets/123</rdfs:comment>
    <rdfs:domain rdf:resource="http://example.org/onto/class/google_bigquery_analytics_hub_listing"/>
    <rdfs:range rdf:resource="http://www.w3.org/2001/XMLSchema#string"/>
  </owl:DatatypeProperty>
  <owl:DatatypeProperty rdf:about="http://example.org/onto/prop/google_bigquery_analytics_hub_listing_table">
    <rdfs:label>table</rdfs:label>
    <rdfs:comment>Format: For table: projects/{projectId}/datasets/{datasetId}/tables/{tableId} Example:"projects/test_project/datasets/test_dataset/tables/test_table"</rdfs:comment>
    <rdfs:domain rdf:resource="http://example.org/onto/class/google_bigquery_analytics_hub_listing"/>
    <rdfs:range rdf:resource="http://www.w3.org/2001/XMLSchema#string"/>
  </owl:DatatypeProperty>
  <owl:DatatypeProperty rdf:about="http://example.org/onto/prop/google_bigquery_analytics_hub_listing_name">
    <rdfs:label>name</rdfs:label>
    <rdfs:comment>Name of the data provider.</rdfs:comment>
    <rdfs:domain rdf:resource="http://example.org/onto/class/google_bigquery_analytics_hub_listing"/>
    <rdfs:range rdf:resource="http://www.w3.org/2001/XMLSchema#string"/>
  </owl:DatatypeProperty>
  <owl:DatatypeProperty rdf:about="http://example.org/onto/prop/google_bigquery_analytics_hub_listing_primary_contact">
    <rdfs:label>primary_contact</rdfs:label>
    <rdfs:comment>Email or URL of the data provider.</rdfs:comment>
    <rdfs:domain rdf:resource="http://example.org/onto/class/google_bigquery_analytics_hub_listing"/>
    <rdfs:range rdf:resource="http://www.w3.org/2001/XMLSchema#string"/>
  </owl:DatatypeProperty>
  <owl:DatatypeProperty rdf:about="http://example.org/onto/prop/google_bigquery_analytics_hub_listing_name">
    <rdfs:label>name</rdfs:label>
    <rdfs:comment>Name of the listing publisher.</rdfs:comment>
    <rdfs:domain rdf:resource="http://example.org/onto/class/google_bigquery_analytics_hub_listing"/>
    <rdfs:range rdf:resource="http://www.w3.org/2001/XMLSchema#string"/>
  </owl:DatatypeProperty>
  <owl:DatatypeProperty rdf:about="http://example.org/onto/prop/google_bigquery_analytics_hub_listing_primary_contact">
    <rdfs:label>primary_contact</rdfs:label>
    <rdfs:comment>Email or URL of the listing publisher.</rdfs:comment>
    <rdfs:domain rdf:resource="http://example.org/onto/class/google_bigquery_analytics_hub_listing"/>
    <rdfs:range rdf:resource="http://www.w3.org/2001/XMLSchema#string"/>
  </owl:DatatypeProperty>
  <owl:DatatypeProperty rdf:about="http://example.org/onto/prop/google_bigquery_analytics_hub_listing_data_affinity_regions">
    <rdfs:label>data_affinity_regions</rdfs:label>
    <rdfs:comment>Region hint on where the data might be published. Data affinity regions are modifiable.
See https://cloud.google.com/about/locations for full listing of possible Cloud regions.</rdfs:comment>
    <rdfs:domain rdf:resource="http://example.org/onto/class/google_bigquery_analytics_hub_listing"/>
    <rdfs:range rdf:resource="http://www.w3.org/2001/XMLSchema#string"/>
  </owl:DatatypeProperty>
  <owl:DatatypeProperty rdf:about="http://example.org/onto/prop/google_bigquery_analytics_hub_listing_topic">
    <rdfs:label>topic</rdfs:label>
    <rdfs:comment>Resource name of the Pub/Sub topic source for this listing. e.g. projects/myproject/topics/topicId</rdfs:comment>
    <rdfs:domain rdf:resource="http://example.org/onto/class/google_bigquery_analytics_hub_listing"/>
    <rdfs:range rdf:resource="http://www.w3.org/2001/XMLSchema#string"/>
  </owl:DatatypeProperty>
  <owl:DatatypeProperty rdf:about="http://example.org/onto/prop/google_bigquery_analytics_hub_listing_enabled">
    <rdfs:label>enabled</rdfs:label>
    <rdfs:comment>If true, enable restricted export.</rdfs:comment>
    <rdfs:domain rdf:resource="http://example.org/onto/class/google_bigquery_analytics_hub_listing"/>
    <rdfs:range rdf:resource="http://www.w3.org/2001/XMLSchema#string"/>
  </owl:DatatypeProperty>
  <owl:DatatypeProperty rdf:about="http://example.org/onto/prop/google_bigquery_analytics_hub_listing_restrict_direct_table_access">
    <rdfs:label>restrict_direct_table_access</rdfs:label>
    <rdfs:comment>If true, restrict direct table access(read api/tabledata.list) on linked table.</rdfs:comment>
    <rdfs:domain rdf:resource="http://example.org/onto/class/google_bigquery_analytics_hub_listing"/>
    <rdfs:range rdf:resource="http://www.w3.org/2001/XMLSchema#string"/>
  </owl:DatatypeProperty>
  <owl:DatatypeProperty rdf:about="http://example.org/onto/prop/google_bigquery_analytics_hub_listing_restrict_query_result">
    <rdfs:label>restrict_query_result</rdfs:label>
    <rdfs:comment>If true, restrict export of query result derived from restricted linked dataset table.</rdfs:comment>
    <rdfs:domain rdf:resource="http://example.org/onto/class/google_bigquery_analytics_hub_listing"/>
    <rdfs:range rdf:resource="http://www.w3.org/2001/XMLSchema#string"/>
  </owl:DatatypeProperty>
  <owl:DatatypeProperty rdf:about="http://example.org/onto/prop/google_bigquery_analytics_hub_listing_create">
    <rdfs:label>create</rdfs:label>
    <rdfs:domain rdf:resource="http://example.org/onto/class/google_bigquery_analytics_hub_listing"/>
    <rdfs:range rdf:resource="http://www.w3.org/2001/XMLSchema#string"/>
  </owl:DatatypeProperty>
  <owl:DatatypeProperty rdf:about="http://example.org/onto/prop/google_bigquery_analytics_hub_listing_delete">
    <rdfs:label>delete</rdfs:label>
    <rdfs:domain rdf:resource="http://example.org/onto/class/google_bigquery_analytics_hub_listing"/>
    <rdfs:range rdf:resource="http://www.w3.org/2001/XMLSchema#string"/>
  </owl:DatatypeProperty>
  <owl:DatatypeProperty rdf:about="http://example.org/onto/prop/google_bigquery_analytics_hub_listing_update">
    <rdfs:label>update</rdfs:label>
    <rdfs:domain rdf:resource="http://example.org/onto/class/google_bigquery_analytics_hub_listing"/>
    <rdfs:range rdf:resource="http://www.w3.org/2001/XMLSchema#string"/>
  </owl:DatatypeProperty>
</rdf:RDF>
