<?xml version="1.0" encoding="UTF-8"?>
<rdf:RDF
  xmlns:rdf="http://www.w3.org/1999/02/22-rdf-syntax-ns#"
  xmlns:rdfs="http://www.w3.org/2000/01/rdf-schema#"
  xmlns:owl="http://www.w3.org/2002/07/owl#"
  xmlns:xsd="http://www.w3.org/2001/XMLSchema#"
  xml:base="http://example.org/onto/">
  <owl:Class rdf:about="http://example.org/onto/class/google_network_security_mirroring_endpoint_group_association">
    <rdfs:label>google_network_security_mirroring_endpoint_group_association</rdfs:label>
    <rdfs:comment>#
#     ***     AUTO GENERATED CODE    ***    Type: MMv1     ***
#
# ----------------------------------------------------------------------------
#
#     This code is generated by Magic Modules using the following:
#
#     Configuration: https:#github.com/GoogleCloudPlatform/magic-modules/tree/main/mmv1/products/networksecurity/MirroringEndpointGroupAssociation.yaml
#     Template:      https:#github.com/GoogleCloudPlatform/magic-modules/tree/main/mmv1/templates/terraform/resource.html.markdown.tmpl
#
#     DO NOT EDIT this file directly. Any changes made to this file will be
#     overwritten during the next generation cycle.
#
# ----------------------------------------------------------------------------
subcategory: "Network Security"
description: |-
  An endpoint group association represents a link between a network and an
  endpoint group in the organization.
---</rdfs:comment>
  </owl:Class>
  <owl:DatatypeProperty rdf:about="http://example.org/onto/prop/google_network_security_mirroring_endpoint_group_association_create_time">
    <rdfs:label>create_time</rdfs:label>
    <rdfs:comment>The timestamp when the resource was created.
See https://google.aip.dev/148#timestamps.</rdfs:comment>
    <rdfs:domain rdf:resource="http://example.org/onto/class/google_network_security_mirroring_endpoint_group_association"/>
    <rdfs:range rdf:resource="http://www.w3.org/2001/XMLSchema#string"/>
  </owl:DatatypeProperty>
  <owl:DatatypeProperty rdf:about="http://example.org/onto/prop/google_network_security_mirroring_endpoint_group_association_effective_labels">
    <rdfs:label>effective_labels</rdfs:label>
    <rdfs:comment>All of labels (key/value pairs) present on the resource in GCP, including the labels configured through Terraform, other clients and services.</rdfs:comment>
    <rdfs:domain rdf:resource="http://example.org/onto/class/google_network_security_mirroring_endpoint_group_association"/>
    <rdfs:range rdf:resource="http://www.w3.org/2001/XMLSchema#string"/>
  </owl:DatatypeProperty>
  <owl:DatatypeProperty rdf:about="http://example.org/onto/prop/google_network_security_mirroring_endpoint_group_association_id">
    <rdfs:label>id</rdfs:label>
    <rdfs:domain rdf:resource="http://example.org/onto/class/google_network_security_mirroring_endpoint_group_association"/>
    <rdfs:range rdf:resource="http://www.w3.org/2001/XMLSchema#string"/>
  </owl:DatatypeProperty>
  <owl:DatatypeProperty rdf:about="http://example.org/onto/prop/google_network_security_mirroring_endpoint_group_association_labels">
    <rdfs:label>labels</rdfs:label>
    <rdfs:comment>Labels are key/value pairs that help to organize and filter resources.

**Note**: This field is non-authoritative, and will only manage the labels present in your configuration.
Please refer to the field 'effective_labels' for all of the labels present on the resource.</rdfs:comment>
    <rdfs:domain rdf:resource="http://example.org/onto/class/google_network_security_mirroring_endpoint_group_association"/>
    <rdfs:range rdf:resource="http://www.w3.org/2001/XMLSchema#string"/>
  </owl:DatatypeProperty>
  <owl:DatatypeProperty rdf:about="http://example.org/onto/prop/google_network_security_mirroring_endpoint_group_association_location">
    <rdfs:label>location</rdfs:label>
    <rdfs:comment>The cloud location of the association, currently restricted to 'global'.</rdfs:comment>
    <rdfs:domain rdf:resource="http://example.org/onto/class/google_network_security_mirroring_endpoint_group_association"/>
    <rdfs:range rdf:resource="http://www.w3.org/2001/XMLSchema#string"/>
  </owl:DatatypeProperty>
  <owl:DatatypeProperty rdf:about="http://example.org/onto/prop/google_network_security_mirroring_endpoint_group_association_locations">
    <rdfs:label>locations</rdfs:label>
    <rdfs:comment>The list of locations where the association is configured. This information
is retrieved from the linked endpoint group.</rdfs:comment>
    <rdfs:domain rdf:resource="http://example.org/onto/class/google_network_security_mirroring_endpoint_group_association"/>
    <rdfs:range rdf:resource="http://www.w3.org/2001/XMLSchema#string"/>
  </owl:DatatypeProperty>
  <owl:DatatypeProperty rdf:about="http://example.org/onto/prop/google_network_security_mirroring_endpoint_group_association_locations_details">
    <rdfs:label>locations_details</rdfs:label>
    <rdfs:comment>The list of locations where the association is present. This information
is retrieved from the linked endpoint group, and not configured as part
of the association itself.</rdfs:comment>
    <rdfs:domain rdf:resource="http://example.org/onto/class/google_network_security_mirroring_endpoint_group_association"/>
    <rdfs:range rdf:resource="http://www.w3.org/2001/XMLSchema#string"/>
  </owl:DatatypeProperty>
  <owl:DatatypeProperty rdf:about="http://example.org/onto/prop/google_network_security_mirroring_endpoint_group_association_mirroring_endpoint_group">
    <rdfs:label>mirroring_endpoint_group</rdfs:label>
    <rdfs:comment>The endpoint group that this association is connected to, for example:
'projects/123456789/locations/global/mirroringEndpointGroups/my-eg'.
See https://google.aip.dev/124.</rdfs:comment>
    <rdfs:domain rdf:resource="http://example.org/onto/class/google_network_security_mirroring_endpoint_group_association"/>
    <rdfs:range rdf:resource="http://www.w3.org/2001/XMLSchema#string"/>
  </owl:DatatypeProperty>
  <owl:DatatypeProperty rdf:about="http://example.org/onto/prop/google_network_security_mirroring_endpoint_group_association_mirroring_endpoint_group_association_id">
    <rdfs:label>mirroring_endpoint_group_association_id</rdfs:label>
    <rdfs:comment>The ID to use for the new association, which will become the final
component of the endpoint group's resource name. If not provided, the
server will generate a unique ID.</rdfs:comment>
    <rdfs:domain rdf:resource="http://example.org/onto/class/google_network_security_mirroring_endpoint_group_association"/>
    <rdfs:range rdf:resource="http://www.w3.org/2001/XMLSchema#string"/>
  </owl:DatatypeProperty>
  <owl:DatatypeProperty rdf:about="http://example.org/onto/prop/google_network_security_mirroring_endpoint_group_association_name">
    <rdfs:label>name</rdfs:label>
    <rdfs:comment>The resource name of this endpoint group association, for example:
'projects/123456789/locations/global/mirroringEndpointGroupAssociations/my-eg-association'.
See https://google.aip.dev/122 for more details.</rdfs:comment>
    <rdfs:domain rdf:resource="http://example.org/onto/class/google_network_security_mirroring_endpoint_group_association"/>
    <rdfs:range rdf:resource="http://www.w3.org/2001/XMLSchema#string"/>
  </owl:DatatypeProperty>
  <owl:DatatypeProperty rdf:about="http://example.org/onto/prop/google_network_security_mirroring_endpoint_group_association_network">
    <rdfs:label>network</rdfs:label>
    <rdfs:comment>The VPC network that is associated. for example:
'projects/123456789/global/networks/my-network'.
See https://google.aip.dev/124.</rdfs:comment>
    <rdfs:domain rdf:resource="http://example.org/onto/class/google_network_security_mirroring_endpoint_group_association"/>
    <rdfs:range rdf:resource="http://www.w3.org/2001/XMLSchema#string"/>
  </owl:DatatypeProperty>
  <owl:DatatypeProperty rdf:about="http://example.org/onto/prop/google_network_security_mirroring_endpoint_group_association_project">
    <rdfs:label>project</rdfs:label>
    <rdfs:domain rdf:resource="http://example.org/onto/class/google_network_security_mirroring_endpoint_group_association"/>
    <rdfs:range rdf:resource="http://www.w3.org/2001/XMLSchema#string"/>
  </owl:DatatypeProperty>
  <owl:DatatypeProperty rdf:about="http://example.org/onto/prop/google_network_security_mirroring_endpoint_group_association_reconciling">
    <rdfs:label>reconciling</rdfs:label>
    <rdfs:comment>The current state of the resource does not match the user's intended state,
and the system is working to reconcile them. This part of the normal
operation (e.g. adding a new location to the target deployment group).
See https://google.aip.dev/128.</rdfs:comment>
    <rdfs:domain rdf:resource="http://example.org/onto/class/google_network_security_mirroring_endpoint_group_association"/>
    <rdfs:range rdf:resource="http://www.w3.org/2001/XMLSchema#string"/>
  </owl:DatatypeProperty>
  <owl:DatatypeProperty rdf:about="http://example.org/onto/prop/google_network_security_mirroring_endpoint_group_association_state">
    <rdfs:label>state</rdfs:label>
    <rdfs:comment>Current state of the endpoint group association.
Possible values:
STATE_UNSPECIFIED
ACTIVE
CREATING
DELETING
CLOSED
OUT_OF_SYNC
DELETE_FAILED</rdfs:comment>
    <rdfs:domain rdf:resource="http://example.org/onto/class/google_network_security_mirroring_endpoint_group_association"/>
    <rdfs:range rdf:resource="http://www.w3.org/2001/XMLSchema#string"/>
  </owl:DatatypeProperty>
  <owl:DatatypeProperty rdf:about="http://example.org/onto/prop/google_network_security_mirroring_endpoint_group_association_terraform_labels">
    <rdfs:label>terraform_labels</rdfs:label>
    <rdfs:comment>The combination of labels configured directly on the resource
 and default labels configured on the provider.</rdfs:comment>
    <rdfs:domain rdf:resource="http://example.org/onto/class/google_network_security_mirroring_endpoint_group_association"/>
    <rdfs:range rdf:resource="http://www.w3.org/2001/XMLSchema#string"/>
  </owl:DatatypeProperty>
  <owl:DatatypeProperty rdf:about="http://example.org/onto/prop/google_network_security_mirroring_endpoint_group_association_update_time">
    <rdfs:label>update_time</rdfs:label>
    <rdfs:comment>The timestamp when the resource was most recently updated.
See https://google.aip.dev/148#timestamps.</rdfs:comment>
    <rdfs:domain rdf:resource="http://example.org/onto/class/google_network_security_mirroring_endpoint_group_association"/>
    <rdfs:range rdf:resource="http://www.w3.org/2001/XMLSchema#string"/>
  </owl:DatatypeProperty>
  <owl:DatatypeProperty rdf:about="http://example.org/onto/prop/google_network_security_mirroring_endpoint_group_association_create">
    <rdfs:label>create</rdfs:label>
    <rdfs:domain rdf:resource="http://example.org/onto/class/google_network_security_mirroring_endpoint_group_association"/>
    <rdfs:range rdf:resource="http://www.w3.org/2001/XMLSchema#string"/>
  </owl:DatatypeProperty>
  <owl:DatatypeProperty rdf:about="http://example.org/onto/prop/google_network_security_mirroring_endpoint_group_association_delete">
    <rdfs:label>delete</rdfs:label>
    <rdfs:domain rdf:resource="http://example.org/onto/class/google_network_security_mirroring_endpoint_group_association"/>
    <rdfs:range rdf:resource="http://www.w3.org/2001/XMLSchema#string"/>
  </owl:DatatypeProperty>
  <owl:DatatypeProperty rdf:about="http://example.org/onto/prop/google_network_security_mirroring_endpoint_group_association_update">
    <rdfs:label>update</rdfs:label>
    <rdfs:domain rdf:resource="http://example.org/onto/class/google_network_security_mirroring_endpoint_group_association"/>
    <rdfs:range rdf:resource="http://www.w3.org/2001/XMLSchema#string"/>
  </owl:DatatypeProperty>
</rdf:RDF>
