<?xml version="1.0" encoding="UTF-8"?>
<rdf:RDF
  xmlns:rdf="http://www.w3.org/1999/02/22-rdf-syntax-ns#"
  xmlns:rdfs="http://www.w3.org/2000/01/rdf-schema#"
  xmlns:owl="http://www.w3.org/2002/07/owl#"
  xmlns:xsd="http://www.w3.org/2001/XMLSchema#"
  xml:base="http://example.org/onto/">
  <owl:Class rdf:about="http://example.org/onto/class/google_compute_target_https_proxy">
    <rdfs:label>google_compute_target_https_proxy</rdfs:label>
    <rdfs:comment>#
#     ***     AUTO GENERATED CODE    ***    Type: MMv1     ***
#
# ----------------------------------------------------------------------------
#
#     This code is generated by Magic Modules using the following:
#
#     Configuration: https:#github.com/GoogleCloudPlatform/magic-modules/tree/main/mmv1/products/compute/TargetHttpsProxy.yaml
#     Template:      https:#github.com/GoogleCloudPlatform/magic-modules/tree/main/mmv1/templates/terraform/resource.html.markdown.tmpl
#
#     DO NOT EDIT this file directly. Any changes made to this file will be
#     overwritten during the next generation cycle.
#
# ----------------------------------------------------------------------------
subcategory: "Compute Engine"
description: |-
  Represents a TargetHttpsProxy resource, which is used by one or more
  global forwarding rule to route incoming HTTPS requests to a URL map.
---</rdfs:comment>
  </owl:Class>
  <owl:DatatypeProperty rdf:about="http://example.org/onto/prop/google_compute_target_https_proxy_certificate_manager_certificates">
    <rdfs:label>certificate_manager_certificates</rdfs:label>
    <rdfs:comment>URLs to certificate manager certificate resources that are used to authenticate connections between users and the load balancer.
Certificate manager certificates only apply when the load balancing scheme is set to INTERNAL_MANAGED.
For EXTERNAL and EXTERNAL_MANAGED, use certificate_map instead.
sslCertificates and certificateManagerCertificates fields can not be defined together.
Accepted format is '//certificatemanager.googleapis.com/projects/{project}/locations/{location}/certificates/{resourceName}' or just the self_link 'projects/{project}/locations/{location}/certificates/{resourceName}'</rdfs:comment>
    <rdfs:domain rdf:resource="http://example.org/onto/class/google_compute_target_https_proxy"/>
    <rdfs:range rdf:resource="http://www.w3.org/2001/XMLSchema#string"/>
  </owl:DatatypeProperty>
  <owl:DatatypeProperty rdf:about="http://example.org/onto/prop/google_compute_target_https_proxy_certificate_map">
    <rdfs:label>certificate_map</rdfs:label>
    <rdfs:comment>A reference to the CertificateMap resource uri that identifies a certificate map
associated with the given target proxy. This field is only supported for EXTERNAL and EXTERNAL_MANAGED load balancing schemes.
For INTERNAL_MANAGED, use certificate_manager_certificates instead.
Accepted format is '//certificatemanager.googleapis.com/projects/{project}/locations/{location}/certificateMaps/{resourceName}'.</rdfs:comment>
    <rdfs:domain rdf:resource="http://example.org/onto/class/google_compute_target_https_proxy"/>
    <rdfs:range rdf:resource="http://www.w3.org/2001/XMLSchema#string"/>
  </owl:DatatypeProperty>
  <owl:DatatypeProperty rdf:about="http://example.org/onto/prop/google_compute_target_https_proxy_creation_timestamp">
    <rdfs:label>creation_timestamp</rdfs:label>
    <rdfs:comment>Creation timestamp in RFC3339 text format.</rdfs:comment>
    <rdfs:domain rdf:resource="http://example.org/onto/class/google_compute_target_https_proxy"/>
    <rdfs:range rdf:resource="http://www.w3.org/2001/XMLSchema#string"/>
  </owl:DatatypeProperty>
  <owl:DatatypeProperty rdf:about="http://example.org/onto/prop/google_compute_target_https_proxy_description">
    <rdfs:label>description</rdfs:label>
    <rdfs:comment>An optional description of this resource.</rdfs:comment>
    <rdfs:domain rdf:resource="http://example.org/onto/class/google_compute_target_https_proxy"/>
    <rdfs:range rdf:resource="http://www.w3.org/2001/XMLSchema#string"/>
  </owl:DatatypeProperty>
  <owl:DatatypeProperty rdf:about="http://example.org/onto/prop/google_compute_target_https_proxy_fingerprint">
    <rdfs:label>fingerprint</rdfs:label>
    <rdfs:comment>Fingerprint of this resource. A hash of the contents stored in this object. This field is used in optimistic locking.
This field will be ignored when inserting a TargetHttpsProxy. An up-to-date fingerprint must be provided in order to
patch the TargetHttpsProxy; otherwise, the request will fail with error 412 conditionNotMet.
To see the latest fingerprint, make a get() request to retrieve the TargetHttpsProxy.
A base64-encoded string.</rdfs:comment>
    <rdfs:domain rdf:resource="http://example.org/onto/class/google_compute_target_https_proxy"/>
    <rdfs:range rdf:resource="http://www.w3.org/2001/XMLSchema#string"/>
  </owl:DatatypeProperty>
  <owl:DatatypeProperty rdf:about="http://example.org/onto/prop/google_compute_target_https_proxy_http_keep_alive_timeout_sec">
    <rdfs:label>http_keep_alive_timeout_sec</rdfs:label>
    <rdfs:comment>Specifies how long to keep a connection open, after completing a response,
while there is no matching traffic (in seconds). If an HTTP keepalive is
not specified, a default value will be used. For Global
external HTTP(S) load balancer, the default value is 610 seconds, the
minimum allowed value is 5 seconds and the maximum allowed value is 1200
seconds. For cross-region internal HTTP(S) load balancer, the default
value is 600 seconds, the minimum allowed value is 5 seconds, and the
maximum allowed value is 600 seconds. For Global external HTTP(S) load
balancer (classic), this option is not available publicly.</rdfs:comment>
    <rdfs:domain rdf:resource="http://example.org/onto/class/google_compute_target_https_proxy"/>
    <rdfs:range rdf:resource="http://www.w3.org/2001/XMLSchema#string"/>
  </owl:DatatypeProperty>
  <owl:DatatypeProperty rdf:about="http://example.org/onto/prop/google_compute_target_https_proxy_id">
    <rdfs:label>id</rdfs:label>
    <rdfs:domain rdf:resource="http://example.org/onto/class/google_compute_target_https_proxy"/>
    <rdfs:range rdf:resource="http://www.w3.org/2001/XMLSchema#string"/>
  </owl:DatatypeProperty>
  <owl:DatatypeProperty rdf:about="http://example.org/onto/prop/google_compute_target_https_proxy_name">
    <rdfs:label>name</rdfs:label>
    <rdfs:comment>Name of the resource. Provided by the client when the resource is
created. The name must be 1-63 characters long, and comply with
RFC1035. Specifically, the name must be 1-63 characters long and match
the regular expression '[a-z]([-a-z0-9]*[a-z0-9])?' which means the
first character must be a lowercase letter, and all following
characters must be a dash, lowercase letter, or digit, except the last
character, which cannot be a dash.</rdfs:comment>
    <rdfs:domain rdf:resource="http://example.org/onto/class/google_compute_target_https_proxy"/>
    <rdfs:range rdf:resource="http://www.w3.org/2001/XMLSchema#string"/>
  </owl:DatatypeProperty>
  <owl:DatatypeProperty rdf:about="http://example.org/onto/prop/google_compute_target_https_proxy_project">
    <rdfs:label>project</rdfs:label>
    <rdfs:domain rdf:resource="http://example.org/onto/class/google_compute_target_https_proxy"/>
    <rdfs:range rdf:resource="http://www.w3.org/2001/XMLSchema#string"/>
  </owl:DatatypeProperty>
  <owl:DatatypeProperty rdf:about="http://example.org/onto/prop/google_compute_target_https_proxy_proxy_bind">
    <rdfs:label>proxy_bind</rdfs:label>
    <rdfs:comment>This field only applies when the forwarding rule that references
this target proxy has a loadBalancingScheme set to INTERNAL_SELF_MANAGED.</rdfs:comment>
    <rdfs:domain rdf:resource="http://example.org/onto/class/google_compute_target_https_proxy"/>
    <rdfs:range rdf:resource="http://www.w3.org/2001/XMLSchema#string"/>
  </owl:DatatypeProperty>
  <owl:DatatypeProperty rdf:about="http://example.org/onto/prop/google_compute_target_https_proxy_proxy_id">
    <rdfs:label>proxy_id</rdfs:label>
    <rdfs:comment>The unique identifier for the resource.</rdfs:comment>
    <rdfs:domain rdf:resource="http://example.org/onto/class/google_compute_target_https_proxy"/>
    <rdfs:range rdf:resource="http://www.w3.org/2001/XMLSchema#string"/>
  </owl:DatatypeProperty>
  <owl:DatatypeProperty rdf:about="http://example.org/onto/prop/google_compute_target_https_proxy_quic_override">
    <rdfs:label>quic_override</rdfs:label>
    <rdfs:comment>Specifies the QUIC override policy for this resource. This determines
whether the load balancer will attempt to negotiate QUIC with clients
or not. Can specify one of NONE, ENABLE, or DISABLE. If NONE is
specified, Google manages whether QUIC is used. Default value: "NONE" Possible values: ["NONE", "ENABLE", "DISABLE"]</rdfs:comment>
    <rdfs:domain rdf:resource="http://example.org/onto/class/google_compute_target_https_proxy"/>
    <rdfs:range rdf:resource="http://www.w3.org/2001/XMLSchema#string"/>
  </owl:DatatypeProperty>
  <owl:DatatypeProperty rdf:about="http://example.org/onto/prop/google_compute_target_https_proxy_self_link">
    <rdfs:label>self_link</rdfs:label>
    <rdfs:domain rdf:resource="http://example.org/onto/class/google_compute_target_https_proxy"/>
    <rdfs:range rdf:resource="http://www.w3.org/2001/XMLSchema#string"/>
  </owl:DatatypeProperty>
  <owl:DatatypeProperty rdf:about="http://example.org/onto/prop/google_compute_target_https_proxy_server_tls_policy">
    <rdfs:label>server_tls_policy</rdfs:label>
    <rdfs:comment>A URL referring to a networksecurity.ServerTlsPolicy
resource that describes how the proxy should authenticate inbound
traffic. serverTlsPolicy only applies to a global TargetHttpsProxy
attached to globalForwardingRules with the loadBalancingScheme
set to INTERNAL_SELF_MANAGED or EXTERNAL or EXTERNAL_MANAGED.
For details which ServerTlsPolicy resources are accepted with
INTERNAL_SELF_MANAGED and which with EXTERNAL, EXTERNAL_MANAGED
loadBalancingScheme consult ServerTlsPolicy documentation.
If left blank, communications are not encrypted.

If you remove this field from your configuration at the same time as
deleting or recreating a referenced ServerTlsPolicy resource, you will
receive a resourceInUseByAnotherResource error. Use lifecycle.create_before_destroy
within the ServerTlsPolicy resource to avoid this.</rdfs:comment>
    <rdfs:domain rdf:resource="http://example.org/onto/class/google_compute_target_https_proxy"/>
    <rdfs:range rdf:resource="http://www.w3.org/2001/XMLSchema#string"/>
  </owl:DatatypeProperty>
  <owl:DatatypeProperty rdf:about="http://example.org/onto/prop/google_compute_target_https_proxy_ssl_certificates">
    <rdfs:label>ssl_certificates</rdfs:label>
    <rdfs:comment>URLs to SslCertificate resources that are used to authenticate connections between users and the load balancer.
Currently, you may specify up to 15 SSL certificates. sslCertificates do not apply when the load balancing scheme is set to INTERNAL_SELF_MANAGED.
sslCertificates and certificateManagerCertificates can not be defined together.</rdfs:comment>
    <rdfs:domain rdf:resource="http://example.org/onto/class/google_compute_target_https_proxy"/>
    <rdfs:range rdf:resource="http://www.w3.org/2001/XMLSchema#string"/>
  </owl:DatatypeProperty>
  <owl:DatatypeProperty rdf:about="http://example.org/onto/prop/google_compute_target_https_proxy_ssl_policy">
    <rdfs:label>ssl_policy</rdfs:label>
    <rdfs:comment>A reference to the SslPolicy resource that will be associated with
the TargetHttpsProxy resource. If not set, the TargetHttpsProxy
resource will not have any SSL policy configured.</rdfs:comment>
    <rdfs:domain rdf:resource="http://example.org/onto/class/google_compute_target_https_proxy"/>
    <rdfs:range rdf:resource="http://www.w3.org/2001/XMLSchema#string"/>
  </owl:DatatypeProperty>
  <owl:DatatypeProperty rdf:about="http://example.org/onto/prop/google_compute_target_https_proxy_tls_early_data">
    <rdfs:label>tls_early_data</rdfs:label>
    <rdfs:comment>Specifies whether TLS 1.3 0-RTT Data (“Early Data”) should be accepted for this service.
Early Data allows a TLS resumption handshake to include the initial application payload
(a HTTP request) alongside the handshake, reducing the effective round trips to “zero”.
This applies to TLS 1.3 connections over TCP (HTTP/2) as well as over UDP (QUIC/h3). Possible values: ["STRICT", "PERMISSIVE", "UNRESTRICTED", "DISABLED"]</rdfs:comment>
    <rdfs:domain rdf:resource="http://example.org/onto/class/google_compute_target_https_proxy"/>
    <rdfs:range rdf:resource="http://www.w3.org/2001/XMLSchema#string"/>
  </owl:DatatypeProperty>
  <owl:DatatypeProperty rdf:about="http://example.org/onto/prop/google_compute_target_https_proxy_url_map">
    <rdfs:label>url_map</rdfs:label>
    <rdfs:comment>A reference to the UrlMap resource that defines the mapping from URL
to the BackendService.</rdfs:comment>
    <rdfs:domain rdf:resource="http://example.org/onto/class/google_compute_target_https_proxy"/>
    <rdfs:range rdf:resource="http://www.w3.org/2001/XMLSchema#string"/>
  </owl:DatatypeProperty>
  <owl:DatatypeProperty rdf:about="http://example.org/onto/prop/google_compute_target_https_proxy_create">
    <rdfs:label>create</rdfs:label>
    <rdfs:domain rdf:resource="http://example.org/onto/class/google_compute_target_https_proxy"/>
    <rdfs:range rdf:resource="http://www.w3.org/2001/XMLSchema#string"/>
  </owl:DatatypeProperty>
  <owl:DatatypeProperty rdf:about="http://example.org/onto/prop/google_compute_target_https_proxy_delete">
    <rdfs:label>delete</rdfs:label>
    <rdfs:domain rdf:resource="http://example.org/onto/class/google_compute_target_https_proxy"/>
    <rdfs:range rdf:resource="http://www.w3.org/2001/XMLSchema#string"/>
  </owl:DatatypeProperty>
  <owl:DatatypeProperty rdf:about="http://example.org/onto/prop/google_compute_target_https_proxy_update">
    <rdfs:label>update</rdfs:label>
    <rdfs:domain rdf:resource="http://example.org/onto/class/google_compute_target_https_proxy"/>
    <rdfs:range rdf:resource="http://www.w3.org/2001/XMLSchema#string"/>
  </owl:DatatypeProperty>
</rdf:RDF>
