<?xml version="1.0" encoding="UTF-8"?>
<rdf:RDF
  xmlns:rdf="http://www.w3.org/1999/02/22-rdf-syntax-ns#"
  xmlns:rdfs="http://www.w3.org/2000/01/rdf-schema#"
  xmlns:owl="http://www.w3.org/2002/07/owl#"
  xmlns:xsd="http://www.w3.org/2001/XMLSchema#"
  xml:base="http://example.org/onto/">
  <owl:Class rdf:about="http://example.org/onto/class/google_redis_instance">
    <rdfs:label>google_redis_instance</rdfs:label>
    <rdfs:comment>#
#     ***     AUTO GENERATED CODE    ***    Type: MMv1     ***
#
# ----------------------------------------------------------------------------
#
#     This code is generated by Magic Modules using the following:
#
#     Configuration: https:#github.com/GoogleCloudPlatform/magic-modules/tree/main/mmv1/products/redis/Instance.yaml
#     Template:      https:#github.com/GoogleCloudPlatform/magic-modules/tree/main/mmv1/templates/terraform/resource.html.markdown.tmpl
#
#     DO NOT EDIT this file directly. Any changes made to this file will be
#     overwritten during the next generation cycle.
#
# ----------------------------------------------------------------------------
subcategory: "Memorystore (Redis)"
description: |-
  A Google Cloud Redis instance.
---</rdfs:comment>
  </owl:Class>
  <owl:DatatypeProperty rdf:about="http://example.org/onto/prop/google_redis_instance_alternative_location_id">
    <rdfs:label>alternative_location_id</rdfs:label>
    <rdfs:comment>Only applicable to STANDARD_HA tier which protects the instance
against zonal failures by provisioning it across two zones.
If provided, it must be a different zone from the one provided in
[locationId].</rdfs:comment>
    <rdfs:domain rdf:resource="http://example.org/onto/class/google_redis_instance"/>
    <rdfs:range rdf:resource="http://www.w3.org/2001/XMLSchema#string"/>
  </owl:DatatypeProperty>
  <owl:DatatypeProperty rdf:about="http://example.org/onto/prop/google_redis_instance_auth_enabled">
    <rdfs:label>auth_enabled</rdfs:label>
    <rdfs:comment>Optional. Indicates whether OSS Redis AUTH is enabled for the
instance. If set to "true" AUTH is enabled on the instance.
Default value is "false" meaning AUTH is disabled.</rdfs:comment>
    <rdfs:domain rdf:resource="http://example.org/onto/class/google_redis_instance"/>
    <rdfs:range rdf:resource="http://www.w3.org/2001/XMLSchema#string"/>
  </owl:DatatypeProperty>
  <owl:DatatypeProperty rdf:about="http://example.org/onto/prop/google_redis_instance_auth_string">
    <rdfs:label>auth_string</rdfs:label>
    <rdfs:comment>AUTH String set on the instance. This field will only be populated if auth_enabled is true.</rdfs:comment>
    <rdfs:domain rdf:resource="http://example.org/onto/class/google_redis_instance"/>
    <rdfs:range rdf:resource="http://www.w3.org/2001/XMLSchema#string"/>
  </owl:DatatypeProperty>
  <owl:DatatypeProperty rdf:about="http://example.org/onto/prop/google_redis_instance_authorized_network">
    <rdfs:label>authorized_network</rdfs:label>
    <rdfs:comment>The full name of the Google Compute Engine network to which the
instance is connected. If left unspecified, the default network
will be used.</rdfs:comment>
    <rdfs:domain rdf:resource="http://example.org/onto/class/google_redis_instance"/>
    <rdfs:range rdf:resource="http://www.w3.org/2001/XMLSchema#string"/>
  </owl:DatatypeProperty>
  <owl:DatatypeProperty rdf:about="http://example.org/onto/prop/google_redis_instance_connect_mode">
    <rdfs:label>connect_mode</rdfs:label>
    <rdfs:comment>The connection mode of the Redis instance. Default value: "DIRECT_PEERING" Possible values: ["DIRECT_PEERING", "PRIVATE_SERVICE_ACCESS"]</rdfs:comment>
    <rdfs:domain rdf:resource="http://example.org/onto/class/google_redis_instance"/>
    <rdfs:range rdf:resource="http://www.w3.org/2001/XMLSchema#string"/>
  </owl:DatatypeProperty>
  <owl:DatatypeProperty rdf:about="http://example.org/onto/prop/google_redis_instance_create_time">
    <rdfs:label>create_time</rdfs:label>
    <rdfs:comment>The time the instance was created in RFC3339 UTC "Zulu" format,
accurate to nanoseconds.</rdfs:comment>
    <rdfs:domain rdf:resource="http://example.org/onto/class/google_redis_instance"/>
    <rdfs:range rdf:resource="http://www.w3.org/2001/XMLSchema#string"/>
  </owl:DatatypeProperty>
  <owl:DatatypeProperty rdf:about="http://example.org/onto/prop/google_redis_instance_current_location_id">
    <rdfs:label>current_location_id</rdfs:label>
    <rdfs:comment>The current zone where the Redis endpoint is placed.
For Basic Tier instances, this will always be the same as the
[locationId] provided by the user at creation time. For Standard Tier
instances, this can be either [locationId] or [alternativeLocationId]
and can change after a failover event.</rdfs:comment>
    <rdfs:domain rdf:resource="http://example.org/onto/class/google_redis_instance"/>
    <rdfs:range rdf:resource="http://www.w3.org/2001/XMLSchema#string"/>
  </owl:DatatypeProperty>
  <owl:DatatypeProperty rdf:about="http://example.org/onto/prop/google_redis_instance_customer_managed_key">
    <rdfs:label>customer_managed_key</rdfs:label>
    <rdfs:comment>Optional. The KMS key reference that you want to use to encrypt the data at rest for this Redis
instance. If this is provided, CMEK is enabled.</rdfs:comment>
    <rdfs:domain rdf:resource="http://example.org/onto/class/google_redis_instance"/>
    <rdfs:range rdf:resource="http://www.w3.org/2001/XMLSchema#string"/>
  </owl:DatatypeProperty>
  <owl:DatatypeProperty rdf:about="http://example.org/onto/prop/google_redis_instance_display_name">
    <rdfs:label>display_name</rdfs:label>
    <rdfs:comment>An arbitrary and optional user-provided name for the instance.</rdfs:comment>
    <rdfs:domain rdf:resource="http://example.org/onto/class/google_redis_instance"/>
    <rdfs:range rdf:resource="http://www.w3.org/2001/XMLSchema#string"/>
  </owl:DatatypeProperty>
  <owl:DatatypeProperty rdf:about="http://example.org/onto/prop/google_redis_instance_effective_labels">
    <rdfs:label>effective_labels</rdfs:label>
    <rdfs:comment>All of labels (key/value pairs) present on the resource in GCP, including the labels configured through Terraform, other clients and services.</rdfs:comment>
    <rdfs:domain rdf:resource="http://example.org/onto/class/google_redis_instance"/>
    <rdfs:range rdf:resource="http://www.w3.org/2001/XMLSchema#string"/>
  </owl:DatatypeProperty>
  <owl:DatatypeProperty rdf:about="http://example.org/onto/prop/google_redis_instance_effective_reserved_ip_range">
    <rdfs:label>effective_reserved_ip_range</rdfs:label>
    <rdfs:comment>The CIDR range of internal addresses that are reserved for this
instance. If not provided, the service will choose an unused /29
block, for example, 10.0.0.0/29 or 192.168.0.0/29. Ranges must be
unique and non-overlapping with existing subnets in an authorized
network.</rdfs:comment>
    <rdfs:domain rdf:resource="http://example.org/onto/class/google_redis_instance"/>
    <rdfs:range rdf:resource="http://www.w3.org/2001/XMLSchema#string"/>
  </owl:DatatypeProperty>
  <owl:DatatypeProperty rdf:about="http://example.org/onto/prop/google_redis_instance_host">
    <rdfs:label>host</rdfs:label>
    <rdfs:comment>Hostname or IP address of the exposed Redis endpoint used by clients
to connect to the service.</rdfs:comment>
    <rdfs:domain rdf:resource="http://example.org/onto/class/google_redis_instance"/>
    <rdfs:range rdf:resource="http://www.w3.org/2001/XMLSchema#string"/>
  </owl:DatatypeProperty>
  <owl:DatatypeProperty rdf:about="http://example.org/onto/prop/google_redis_instance_id">
    <rdfs:label>id</rdfs:label>
    <rdfs:domain rdf:resource="http://example.org/onto/class/google_redis_instance"/>
    <rdfs:range rdf:resource="http://www.w3.org/2001/XMLSchema#string"/>
  </owl:DatatypeProperty>
  <owl:DatatypeProperty rdf:about="http://example.org/onto/prop/google_redis_instance_labels">
    <rdfs:label>labels</rdfs:label>
    <rdfs:comment>Resource labels to represent user provided metadata.

**Note**: This field is non-authoritative, and will only manage the labels present in your configuration.
Please refer to the field 'effective_labels' for all of the labels present on the resource.</rdfs:comment>
    <rdfs:domain rdf:resource="http://example.org/onto/class/google_redis_instance"/>
    <rdfs:range rdf:resource="http://www.w3.org/2001/XMLSchema#string"/>
  </owl:DatatypeProperty>
  <owl:DatatypeProperty rdf:about="http://example.org/onto/prop/google_redis_instance_location_id">
    <rdfs:label>location_id</rdfs:label>
    <rdfs:comment>The zone where the instance will be provisioned. If not provided,
the service will choose a zone for the instance. For STANDARD_HA tier,
instances will be created across two zones for protection against
zonal failures. If [alternativeLocationId] is also provided, it must
be different from [locationId].</rdfs:comment>
    <rdfs:domain rdf:resource="http://example.org/onto/class/google_redis_instance"/>
    <rdfs:range rdf:resource="http://www.w3.org/2001/XMLSchema#string"/>
  </owl:DatatypeProperty>
  <owl:DatatypeProperty rdf:about="http://example.org/onto/prop/google_redis_instance_maintenance_schedule">
    <rdfs:label>maintenance_schedule</rdfs:label>
    <rdfs:comment>Upcoming maintenance schedule.</rdfs:comment>
    <rdfs:domain rdf:resource="http://example.org/onto/class/google_redis_instance"/>
    <rdfs:range rdf:resource="http://www.w3.org/2001/XMLSchema#string"/>
  </owl:DatatypeProperty>
  <owl:DatatypeProperty rdf:about="http://example.org/onto/prop/google_redis_instance_maintenance_version">
    <rdfs:label>maintenance_version</rdfs:label>
    <rdfs:comment>The self service update maintenance version.</rdfs:comment>
    <rdfs:domain rdf:resource="http://example.org/onto/class/google_redis_instance"/>
    <rdfs:range rdf:resource="http://www.w3.org/2001/XMLSchema#string"/>
  </owl:DatatypeProperty>
  <owl:DatatypeProperty rdf:about="http://example.org/onto/prop/google_redis_instance_memory_size_gb">
    <rdfs:label>memory_size_gb</rdfs:label>
    <rdfs:comment>Redis memory size in GiB.</rdfs:comment>
    <rdfs:domain rdf:resource="http://example.org/onto/class/google_redis_instance"/>
    <rdfs:range rdf:resource="http://www.w3.org/2001/XMLSchema#string"/>
  </owl:DatatypeProperty>
  <owl:DatatypeProperty rdf:about="http://example.org/onto/prop/google_redis_instance_name">
    <rdfs:label>name</rdfs:label>
    <rdfs:comment>The ID of the instance or a fully qualified identifier for the instance.</rdfs:comment>
    <rdfs:domain rdf:resource="http://example.org/onto/class/google_redis_instance"/>
    <rdfs:range rdf:resource="http://www.w3.org/2001/XMLSchema#string"/>
  </owl:DatatypeProperty>
  <owl:DatatypeProperty rdf:about="http://example.org/onto/prop/google_redis_instance_nodes">
    <rdfs:label>nodes</rdfs:label>
    <rdfs:comment>Output only. Info per node.</rdfs:comment>
    <rdfs:domain rdf:resource="http://example.org/onto/class/google_redis_instance"/>
    <rdfs:range rdf:resource="http://www.w3.org/2001/XMLSchema#string"/>
  </owl:DatatypeProperty>
  <owl:DatatypeProperty rdf:about="http://example.org/onto/prop/google_redis_instance_persistence_iam_identity">
    <rdfs:label>persistence_iam_identity</rdfs:label>
    <rdfs:comment>Output only. Cloud IAM identity used by import / export operations
to transfer data to/from Cloud Storage. Format is "serviceAccount:".
The value may change over time for a given instance so should be
checked before each import/export operation.</rdfs:comment>
    <rdfs:domain rdf:resource="http://example.org/onto/class/google_redis_instance"/>
    <rdfs:range rdf:resource="http://www.w3.org/2001/XMLSchema#string"/>
  </owl:DatatypeProperty>
  <owl:DatatypeProperty rdf:about="http://example.org/onto/prop/google_redis_instance_port">
    <rdfs:label>port</rdfs:label>
    <rdfs:comment>The port number of the exposed Redis endpoint.</rdfs:comment>
    <rdfs:domain rdf:resource="http://example.org/onto/class/google_redis_instance"/>
    <rdfs:range rdf:resource="http://www.w3.org/2001/XMLSchema#string"/>
  </owl:DatatypeProperty>
  <owl:DatatypeProperty rdf:about="http://example.org/onto/prop/google_redis_instance_project">
    <rdfs:label>project</rdfs:label>
    <rdfs:domain rdf:resource="http://example.org/onto/class/google_redis_instance"/>
    <rdfs:range rdf:resource="http://www.w3.org/2001/XMLSchema#string"/>
  </owl:DatatypeProperty>
  <owl:DatatypeProperty rdf:about="http://example.org/onto/prop/google_redis_instance_read_endpoint">
    <rdfs:label>read_endpoint</rdfs:label>
    <rdfs:comment>Output only. Hostname or IP address of the exposed readonly Redis endpoint. Standard tier only.
Targets all healthy replica nodes in instance. Replication is asynchronous and replica nodes
will exhibit some lag behind the primary. Write requests must target 'host'.</rdfs:comment>
    <rdfs:domain rdf:resource="http://example.org/onto/class/google_redis_instance"/>
    <rdfs:range rdf:resource="http://www.w3.org/2001/XMLSchema#string"/>
  </owl:DatatypeProperty>
  <owl:DatatypeProperty rdf:about="http://example.org/onto/prop/google_redis_instance_read_endpoint_port">
    <rdfs:label>read_endpoint_port</rdfs:label>
    <rdfs:comment>Output only. The port number of the exposed readonly redis endpoint. Standard tier only.
Write requests should target 'port'.</rdfs:comment>
    <rdfs:domain rdf:resource="http://example.org/onto/class/google_redis_instance"/>
    <rdfs:range rdf:resource="http://www.w3.org/2001/XMLSchema#string"/>
  </owl:DatatypeProperty>
  <owl:DatatypeProperty rdf:about="http://example.org/onto/prop/google_redis_instance_read_replicas_mode">
    <rdfs:label>read_replicas_mode</rdfs:label>
    <rdfs:comment>Optional. Read replica mode. Can only be specified when trying to create the instance.
If not set, Memorystore Redis backend will default to READ_REPLICAS_DISABLED.
- READ_REPLICAS_DISABLED: If disabled, read endpoint will not be provided and the
instance cannot scale up or down the number of replicas.
- READ_REPLICAS_ENABLED: If enabled, read endpoint will be provided and the instance
can scale up and down the number of replicas. Possible values: ["READ_REPLICAS_DISABLED", "READ_REPLICAS_ENABLED"]</rdfs:comment>
    <rdfs:domain rdf:resource="http://example.org/onto/class/google_redis_instance"/>
    <rdfs:range rdf:resource="http://www.w3.org/2001/XMLSchema#string"/>
  </owl:DatatypeProperty>
  <owl:DatatypeProperty rdf:about="http://example.org/onto/prop/google_redis_instance_redis_configs">
    <rdfs:label>redis_configs</rdfs:label>
    <rdfs:comment>Redis configuration parameters, according to http://redis.io/topics/config.
Please check Memorystore documentation for the list of supported parameters:
https://cloud.google.com/memorystore/docs/redis/reference/rest/v1/projects.locations.instances#Instance.FIELDS.redis_configs</rdfs:comment>
    <rdfs:domain rdf:resource="http://example.org/onto/class/google_redis_instance"/>
    <rdfs:range rdf:resource="http://www.w3.org/2001/XMLSchema#string"/>
  </owl:DatatypeProperty>
  <owl:DatatypeProperty rdf:about="http://example.org/onto/prop/google_redis_instance_redis_version">
    <rdfs:label>redis_version</rdfs:label>
    <rdfs:comment>The version of Redis software. If not provided, latest supported
version will be used. Please check the API documentation linked
at the top for the latest valid values.</rdfs:comment>
    <rdfs:domain rdf:resource="http://example.org/onto/class/google_redis_instance"/>
    <rdfs:range rdf:resource="http://www.w3.org/2001/XMLSchema#string"/>
  </owl:DatatypeProperty>
  <owl:DatatypeProperty rdf:about="http://example.org/onto/prop/google_redis_instance_region">
    <rdfs:label>region</rdfs:label>
    <rdfs:comment>The name of the Redis region of the instance.</rdfs:comment>
    <rdfs:domain rdf:resource="http://example.org/onto/class/google_redis_instance"/>
    <rdfs:range rdf:resource="http://www.w3.org/2001/XMLSchema#string"/>
  </owl:DatatypeProperty>
  <owl:DatatypeProperty rdf:about="http://example.org/onto/prop/google_redis_instance_replica_count">
    <rdfs:label>replica_count</rdfs:label>
    <rdfs:comment>Optional. The number of replica nodes. The valid range for the Standard Tier with
read replicas enabled is [1-5] and defaults to 2. If read replicas are not enabled
for a Standard Tier instance, the only valid value is 1 and the default is 1.
The valid value for basic tier is 0 and the default is also 0.</rdfs:comment>
    <rdfs:domain rdf:resource="http://example.org/onto/class/google_redis_instance"/>
    <rdfs:range rdf:resource="http://www.w3.org/2001/XMLSchema#string"/>
  </owl:DatatypeProperty>
  <owl:DatatypeProperty rdf:about="http://example.org/onto/prop/google_redis_instance_reserved_ip_range">
    <rdfs:label>reserved_ip_range</rdfs:label>
    <rdfs:comment>The CIDR range of internal addresses that are reserved for this
instance. If not provided, the service will choose an unused /29
block, for example, 10.0.0.0/29 or 192.168.0.0/29. Ranges must be
unique and non-overlapping with existing subnets in an authorized
network.</rdfs:comment>
    <rdfs:domain rdf:resource="http://example.org/onto/class/google_redis_instance"/>
    <rdfs:range rdf:resource="http://www.w3.org/2001/XMLSchema#string"/>
  </owl:DatatypeProperty>
  <owl:DatatypeProperty rdf:about="http://example.org/onto/prop/google_redis_instance_secondary_ip_range">
    <rdfs:label>secondary_ip_range</rdfs:label>
    <rdfs:comment>Optional. Additional IP range for node placement. Required when enabling read replicas on
an existing instance. For DIRECT_PEERING mode value must be a CIDR range of size /28, or
"auto". For PRIVATE_SERVICE_ACCESS mode value must be the name of an allocated address
range associated with the private service access connection, or "auto".</rdfs:comment>
    <rdfs:domain rdf:resource="http://example.org/onto/class/google_redis_instance"/>
    <rdfs:range rdf:resource="http://www.w3.org/2001/XMLSchema#string"/>
  </owl:DatatypeProperty>
  <owl:DatatypeProperty rdf:about="http://example.org/onto/prop/google_redis_instance_server_ca_certs">
    <rdfs:label>server_ca_certs</rdfs:label>
    <rdfs:comment>List of server CA certificates for the instance.</rdfs:comment>
    <rdfs:domain rdf:resource="http://example.org/onto/class/google_redis_instance"/>
    <rdfs:range rdf:resource="http://www.w3.org/2001/XMLSchema#string"/>
  </owl:DatatypeProperty>
  <owl:DatatypeProperty rdf:about="http://example.org/onto/prop/google_redis_instance_terraform_labels">
    <rdfs:label>terraform_labels</rdfs:label>
    <rdfs:comment>The combination of labels configured directly on the resource
 and default labels configured on the provider.</rdfs:comment>
    <rdfs:domain rdf:resource="http://example.org/onto/class/google_redis_instance"/>
    <rdfs:range rdf:resource="http://www.w3.org/2001/XMLSchema#string"/>
  </owl:DatatypeProperty>
  <owl:DatatypeProperty rdf:about="http://example.org/onto/prop/google_redis_instance_tier">
    <rdfs:label>tier</rdfs:label>
    <rdfs:comment>The service tier of the instance. Must be one of these values:

- BASIC: standalone instance
- STANDARD_HA: highly available primary/replica instances Default value: "BASIC" Possible values: ["BASIC", "STANDARD_HA"]</rdfs:comment>
    <rdfs:domain rdf:resource="http://example.org/onto/class/google_redis_instance"/>
    <rdfs:range rdf:resource="http://www.w3.org/2001/XMLSchema#string"/>
  </owl:DatatypeProperty>
  <owl:DatatypeProperty rdf:about="http://example.org/onto/prop/google_redis_instance_transit_encryption_mode">
    <rdfs:label>transit_encryption_mode</rdfs:label>
    <rdfs:comment>The TLS mode of the Redis instance, If not provided, TLS is disabled for the instance.

- SERVER_AUTHENTICATION: Client to Server traffic encryption enabled with server authentication Default value: "DISABLED" Possible values: ["SERVER_AUTHENTICATION", "DISABLED"]</rdfs:comment>
    <rdfs:domain rdf:resource="http://example.org/onto/class/google_redis_instance"/>
    <rdfs:range rdf:resource="http://www.w3.org/2001/XMLSchema#string"/>
  </owl:DatatypeProperty>
  <owl:DatatypeProperty rdf:about="http://example.org/onto/prop/google_redis_instance_create_time">
    <rdfs:label>create_time</rdfs:label>
    <rdfs:comment>Output only. The time when the policy was created.
A timestamp in RFC3339 UTC "Zulu" format, with nanosecond
resolution and up to nine fractional digits.</rdfs:comment>
    <rdfs:domain rdf:resource="http://example.org/onto/class/google_redis_instance"/>
    <rdfs:range rdf:resource="http://www.w3.org/2001/XMLSchema#string"/>
  </owl:DatatypeProperty>
  <owl:DatatypeProperty rdf:about="http://example.org/onto/prop/google_redis_instance_description">
    <rdfs:label>description</rdfs:label>
    <rdfs:comment>Optional. Description of what this policy is for.
Create/Update methods return INVALID_ARGUMENT if the
length is greater than 512.</rdfs:comment>
    <rdfs:domain rdf:resource="http://example.org/onto/class/google_redis_instance"/>
    <rdfs:range rdf:resource="http://www.w3.org/2001/XMLSchema#string"/>
  </owl:DatatypeProperty>
  <owl:DatatypeProperty rdf:about="http://example.org/onto/prop/google_redis_instance_update_time">
    <rdfs:label>update_time</rdfs:label>
    <rdfs:comment>Output only. The time when the policy was last updated.
A timestamp in RFC3339 UTC "Zulu" format, with nanosecond
resolution and up to nine fractional digits.</rdfs:comment>
    <rdfs:domain rdf:resource="http://example.org/onto/class/google_redis_instance"/>
    <rdfs:range rdf:resource="http://www.w3.org/2001/XMLSchema#string"/>
  </owl:DatatypeProperty>
  <owl:DatatypeProperty rdf:about="http://example.org/onto/prop/google_redis_instance_day">
    <rdfs:label>day</rdfs:label>
    <rdfs:comment>Required. The day of week that maintenance updates occur.

- DAY_OF_WEEK_UNSPECIFIED: The day of the week is unspecified.
- MONDAY: Monday
- TUESDAY: Tuesday
- WEDNESDAY: Wednesday
- THURSDAY: Thursday
- FRIDAY: Friday
- SATURDAY: Saturday
- SUNDAY: Sunday Possible values: ["DAY_OF_WEEK_UNSPECIFIED", "MONDAY", "TUESDAY", "WEDNESDAY", "THURSDAY", "FRIDAY", "SATURDAY", "SUNDAY"]</rdfs:comment>
    <rdfs:domain rdf:resource="http://example.org/onto/class/google_redis_instance"/>
    <rdfs:range rdf:resource="http://www.w3.org/2001/XMLSchema#string"/>
  </owl:DatatypeProperty>
  <owl:DatatypeProperty rdf:about="http://example.org/onto/prop/google_redis_instance_duration">
    <rdfs:label>duration</rdfs:label>
    <rdfs:comment>Output only. Duration of the maintenance window.
The current window is fixed at 1 hour.
A duration in seconds with up to nine fractional digits,
terminated by 's'. Example: "3.5s".</rdfs:comment>
    <rdfs:domain rdf:resource="http://example.org/onto/class/google_redis_instance"/>
    <rdfs:range rdf:resource="http://www.w3.org/2001/XMLSchema#string"/>
  </owl:DatatypeProperty>
  <owl:DatatypeProperty rdf:about="http://example.org/onto/prop/google_redis_instance_hours">
    <rdfs:label>hours</rdfs:label>
    <rdfs:comment>Hours of day in 24 hour format. Should be from 0 to 23.
An API may choose to allow the value "24:00:00" for scenarios like business closing time.</rdfs:comment>
    <rdfs:domain rdf:resource="http://example.org/onto/class/google_redis_instance"/>
    <rdfs:range rdf:resource="http://www.w3.org/2001/XMLSchema#string"/>
  </owl:DatatypeProperty>
  <owl:DatatypeProperty rdf:about="http://example.org/onto/prop/google_redis_instance_minutes">
    <rdfs:label>minutes</rdfs:label>
    <rdfs:comment>Minutes of hour of day. Must be from 0 to 59.</rdfs:comment>
    <rdfs:domain rdf:resource="http://example.org/onto/class/google_redis_instance"/>
    <rdfs:range rdf:resource="http://www.w3.org/2001/XMLSchema#string"/>
  </owl:DatatypeProperty>
  <owl:DatatypeProperty rdf:about="http://example.org/onto/prop/google_redis_instance_nanos">
    <rdfs:label>nanos</rdfs:label>
    <rdfs:comment>Fractions of seconds in nanoseconds. Must be from 0 to 999,999,999.</rdfs:comment>
    <rdfs:domain rdf:resource="http://example.org/onto/class/google_redis_instance"/>
    <rdfs:range rdf:resource="http://www.w3.org/2001/XMLSchema#string"/>
  </owl:DatatypeProperty>
  <owl:DatatypeProperty rdf:about="http://example.org/onto/prop/google_redis_instance_seconds">
    <rdfs:label>seconds</rdfs:label>
    <rdfs:comment>Seconds of minutes of the time. Must normally be from 0 to 59.
An API may allow the value 60 if it allows leap-seconds.</rdfs:comment>
    <rdfs:domain rdf:resource="http://example.org/onto/class/google_redis_instance"/>
    <rdfs:range rdf:resource="http://www.w3.org/2001/XMLSchema#string"/>
  </owl:DatatypeProperty>
  <owl:DatatypeProperty rdf:about="http://example.org/onto/prop/google_redis_instance_persistence_mode">
    <rdfs:label>persistence_mode</rdfs:label>
    <rdfs:comment>Optional. Controls whether Persistence features are enabled. If not provided, the existing value will be used.

- DISABLED: 	Persistence is disabled for the instance, and any existing snapshots are deleted.
- RDB: RDB based Persistence is enabled. Possible values: ["DISABLED", "RDB"]</rdfs:comment>
    <rdfs:domain rdf:resource="http://example.org/onto/class/google_redis_instance"/>
    <rdfs:range rdf:resource="http://www.w3.org/2001/XMLSchema#string"/>
  </owl:DatatypeProperty>
  <owl:DatatypeProperty rdf:about="http://example.org/onto/prop/google_redis_instance_rdb_next_snapshot_time">
    <rdfs:label>rdb_next_snapshot_time</rdfs:label>
    <rdfs:comment>Output only. The next time that a snapshot attempt is scheduled to occur.
A timestamp in RFC3339 UTC "Zulu" format, with nanosecond resolution and up
to nine fractional digits.
Examples: "2014-10-02T15:01:23Z" and "2014-10-02T15:01:23.045123456Z".</rdfs:comment>
    <rdfs:domain rdf:resource="http://example.org/onto/class/google_redis_instance"/>
    <rdfs:range rdf:resource="http://www.w3.org/2001/XMLSchema#string"/>
  </owl:DatatypeProperty>
  <owl:DatatypeProperty rdf:about="http://example.org/onto/prop/google_redis_instance_rdb_snapshot_period">
    <rdfs:label>rdb_snapshot_period</rdfs:label>
    <rdfs:comment>Optional. Available snapshot periods for scheduling.

- ONE_HOUR:	Snapshot every 1 hour.
- SIX_HOURS:	Snapshot every 6 hours.
- TWELVE_HOURS:	Snapshot every 12 hours.
- TWENTY_FOUR_HOURS:	Snapshot every 24 hours. Possible values: ["ONE_HOUR", "SIX_HOURS", "TWELVE_HOURS", "TWENTY_FOUR_HOURS"]</rdfs:comment>
    <rdfs:domain rdf:resource="http://example.org/onto/class/google_redis_instance"/>
    <rdfs:range rdf:resource="http://www.w3.org/2001/XMLSchema#string"/>
  </owl:DatatypeProperty>
  <owl:DatatypeProperty rdf:about="http://example.org/onto/prop/google_redis_instance_rdb_snapshot_start_time">
    <rdfs:label>rdb_snapshot_start_time</rdfs:label>
    <rdfs:comment>Optional. Date and time that the first snapshot was/will be attempted,
and to which future snapshots will be aligned. If not provided,
the current time will be used.
A timestamp in RFC3339 UTC "Zulu" format, with nanosecond resolution
and up to nine fractional digits.
Examples: "2014-10-02T15:01:23Z" and "2014-10-02T15:01:23.045123456Z".</rdfs:comment>
    <rdfs:domain rdf:resource="http://example.org/onto/class/google_redis_instance"/>
    <rdfs:range rdf:resource="http://www.w3.org/2001/XMLSchema#string"/>
  </owl:DatatypeProperty>
  <owl:DatatypeProperty rdf:about="http://example.org/onto/prop/google_redis_instance_create">
    <rdfs:label>create</rdfs:label>
    <rdfs:domain rdf:resource="http://example.org/onto/class/google_redis_instance"/>
    <rdfs:range rdf:resource="http://www.w3.org/2001/XMLSchema#string"/>
  </owl:DatatypeProperty>
  <owl:DatatypeProperty rdf:about="http://example.org/onto/prop/google_redis_instance_delete">
    <rdfs:label>delete</rdfs:label>
    <rdfs:domain rdf:resource="http://example.org/onto/class/google_redis_instance"/>
    <rdfs:range rdf:resource="http://www.w3.org/2001/XMLSchema#string"/>
  </owl:DatatypeProperty>
  <owl:DatatypeProperty rdf:about="http://example.org/onto/prop/google_redis_instance_update">
    <rdfs:label>update</rdfs:label>
    <rdfs:domain rdf:resource="http://example.org/onto/class/google_redis_instance"/>
    <rdfs:range rdf:resource="http://www.w3.org/2001/XMLSchema#string"/>
  </owl:DatatypeProperty>
</rdf:RDF>
