<?xml version="1.0" encoding="UTF-8"?>
<rdf:RDF
  xmlns:rdf="http://www.w3.org/1999/02/22-rdf-syntax-ns#"
  xmlns:rdfs="http://www.w3.org/2000/01/rdf-schema#"
  xmlns:owl="http://www.w3.org/2002/07/owl#"
  xmlns:xsd="http://www.w3.org/2001/XMLSchema#"
  xml:base="http://example.org/onto/">
  <owl:Class rdf:about="http://example.org/onto/class/google_colab_schedule">
    <rdfs:label>google_colab_schedule</rdfs:label>
    <rdfs:comment>#
#     ***     AUTO GENERATED CODE    ***    Type: MMv1     ***
#
# ----------------------------------------------------------------------------
#
#     This code is generated by Magic Modules using the following:
#
#     Configuration: https:#github.com/GoogleCloudPlatform/magic-modules/tree/main/mmv1/products/colab/Schedule.yaml
#     Template:      https:#github.com/GoogleCloudPlatform/magic-modules/tree/main/mmv1/templates/terraform/resource.html.markdown.tmpl
#
#     DO NOT EDIT this file directly. Any changes made to this file will be
#     overwritten during the next generation cycle.
#
# ----------------------------------------------------------------------------
subcategory: "Colab Enterprise"
description: |-
  'Colab Enterprise Notebook Execution Schedules.
---</rdfs:comment>
  </owl:Class>
  <owl:DatatypeProperty rdf:about="http://example.org/onto/prop/google_colab_schedule_allow_queueing">
    <rdfs:label>allow_queueing</rdfs:label>
    <rdfs:comment>Whether new scheduled runs can be queued when max_concurrent_runs limit is reached. If set to true, new runs will be queued instead of skipped. Default to false.</rdfs:comment>
    <rdfs:domain rdf:resource="http://example.org/onto/class/google_colab_schedule"/>
    <rdfs:range rdf:resource="http://www.w3.org/2001/XMLSchema#string"/>
  </owl:DatatypeProperty>
  <owl:DatatypeProperty rdf:about="http://example.org/onto/prop/google_colab_schedule_cron">
    <rdfs:label>cron</rdfs:label>
    <rdfs:comment>Cron schedule (https://en.wikipedia.org/wiki/Cron) to launch scheduled runs.</rdfs:comment>
    <rdfs:domain rdf:resource="http://example.org/onto/class/google_colab_schedule"/>
    <rdfs:range rdf:resource="http://www.w3.org/2001/XMLSchema#string"/>
  </owl:DatatypeProperty>
  <owl:DatatypeProperty rdf:about="http://example.org/onto/prop/google_colab_schedule_desired_state">
    <rdfs:label>desired_state</rdfs:label>
    <rdfs:comment>Desired state of the Colab Schedule. Set this field to 'ACTIVE' to start/resume the schedule, and 'PAUSED' to pause the schedule.</rdfs:comment>
    <rdfs:domain rdf:resource="http://example.org/onto/class/google_colab_schedule"/>
    <rdfs:range rdf:resource="http://www.w3.org/2001/XMLSchema#string"/>
  </owl:DatatypeProperty>
  <owl:DatatypeProperty rdf:about="http://example.org/onto/prop/google_colab_schedule_display_name">
    <rdfs:label>display_name</rdfs:label>
    <rdfs:comment>Required. The display name of the Schedule.</rdfs:comment>
    <rdfs:domain rdf:resource="http://example.org/onto/class/google_colab_schedule"/>
    <rdfs:range rdf:resource="http://www.w3.org/2001/XMLSchema#string"/>
  </owl:DatatypeProperty>
  <owl:DatatypeProperty rdf:about="http://example.org/onto/prop/google_colab_schedule_end_time">
    <rdfs:label>end_time</rdfs:label>
    <rdfs:comment>Timestamp after which no new runs can be scheduled. If specified, the schedule will be completed when either end_time is reached or when scheduled_run_count >= max_run_count. Must be in the RFC 3339 (https://www.ietf.org/rfc/rfc3339.txt) format.</rdfs:comment>
    <rdfs:domain rdf:resource="http://example.org/onto/class/google_colab_schedule"/>
    <rdfs:range rdf:resource="http://www.w3.org/2001/XMLSchema#string"/>
  </owl:DatatypeProperty>
  <owl:DatatypeProperty rdf:about="http://example.org/onto/prop/google_colab_schedule_id">
    <rdfs:label>id</rdfs:label>
    <rdfs:domain rdf:resource="http://example.org/onto/class/google_colab_schedule"/>
    <rdfs:range rdf:resource="http://www.w3.org/2001/XMLSchema#string"/>
  </owl:DatatypeProperty>
  <owl:DatatypeProperty rdf:about="http://example.org/onto/prop/google_colab_schedule_location">
    <rdfs:label>location</rdfs:label>
    <rdfs:comment>The location for the resource: https://cloud.google.com/colab/docs/locations</rdfs:comment>
    <rdfs:domain rdf:resource="http://example.org/onto/class/google_colab_schedule"/>
    <rdfs:range rdf:resource="http://www.w3.org/2001/XMLSchema#string"/>
  </owl:DatatypeProperty>
  <owl:DatatypeProperty rdf:about="http://example.org/onto/prop/google_colab_schedule_max_concurrent_run_count">
    <rdfs:label>max_concurrent_run_count</rdfs:label>
    <rdfs:comment>Maximum number of runs that can be started concurrently for this Schedule. This is the limit for starting the scheduled requests and not the execution of the notebook execution jobs created by the requests.</rdfs:comment>
    <rdfs:domain rdf:resource="http://example.org/onto/class/google_colab_schedule"/>
    <rdfs:range rdf:resource="http://www.w3.org/2001/XMLSchema#string"/>
  </owl:DatatypeProperty>
  <owl:DatatypeProperty rdf:about="http://example.org/onto/prop/google_colab_schedule_max_run_count">
    <rdfs:label>max_run_count</rdfs:label>
    <rdfs:comment>Maximum run count of the schedule. If specified, The schedule will be completed when either startedRunCount >= maxRunCount or when endTime is reached. If not specified, new runs will keep getting scheduled until this Schedule is paused or deleted. Already scheduled runs will be allowed to complete. Unset if not specified.</rdfs:comment>
    <rdfs:domain rdf:resource="http://example.org/onto/class/google_colab_schedule"/>
    <rdfs:range rdf:resource="http://www.w3.org/2001/XMLSchema#string"/>
  </owl:DatatypeProperty>
  <owl:DatatypeProperty rdf:about="http://example.org/onto/prop/google_colab_schedule_name">
    <rdfs:label>name</rdfs:label>
    <rdfs:comment>The resource name of the Schedule</rdfs:comment>
    <rdfs:domain rdf:resource="http://example.org/onto/class/google_colab_schedule"/>
    <rdfs:range rdf:resource="http://www.w3.org/2001/XMLSchema#string"/>
  </owl:DatatypeProperty>
  <owl:DatatypeProperty rdf:about="http://example.org/onto/prop/google_colab_schedule_project">
    <rdfs:label>project</rdfs:label>
    <rdfs:domain rdf:resource="http://example.org/onto/class/google_colab_schedule"/>
    <rdfs:range rdf:resource="http://www.w3.org/2001/XMLSchema#string"/>
  </owl:DatatypeProperty>
  <owl:DatatypeProperty rdf:about="http://example.org/onto/prop/google_colab_schedule_start_time">
    <rdfs:label>start_time</rdfs:label>
    <rdfs:comment>The timestamp after which the first run can be scheduled. Defaults to the schedule creation time. Must be in the RFC 3339 (https://www.ietf.org/rfc/rfc3339.txt) format.</rdfs:comment>
    <rdfs:domain rdf:resource="http://example.org/onto/class/google_colab_schedule"/>
    <rdfs:range rdf:resource="http://www.w3.org/2001/XMLSchema#string"/>
  </owl:DatatypeProperty>
  <owl:DatatypeProperty rdf:about="http://example.org/onto/prop/google_colab_schedule_state">
    <rdfs:label>state</rdfs:label>
    <rdfs:comment>Output only. The state of the schedule.</rdfs:comment>
    <rdfs:domain rdf:resource="http://example.org/onto/class/google_colab_schedule"/>
    <rdfs:range rdf:resource="http://www.w3.org/2001/XMLSchema#string"/>
  </owl:DatatypeProperty>
  <owl:DatatypeProperty rdf:about="http://example.org/onto/prop/google_colab_schedule_display_name">
    <rdfs:label>display_name</rdfs:label>
    <rdfs:comment>Required. The display name of the Notebook Execution.</rdfs:comment>
    <rdfs:domain rdf:resource="http://example.org/onto/class/google_colab_schedule"/>
    <rdfs:range rdf:resource="http://www.w3.org/2001/XMLSchema#string"/>
  </owl:DatatypeProperty>
  <owl:DatatypeProperty rdf:about="http://example.org/onto/prop/google_colab_schedule_execution_timeout">
    <rdfs:label>execution_timeout</rdfs:label>
    <rdfs:comment>Max running time of the execution job in seconds (default 86400s / 24 hrs). A duration in seconds with up to nine fractional digits, ending with "s". Example: "3.5s".</rdfs:comment>
    <rdfs:domain rdf:resource="http://example.org/onto/class/google_colab_schedule"/>
    <rdfs:range rdf:resource="http://www.w3.org/2001/XMLSchema#string"/>
  </owl:DatatypeProperty>
  <owl:DatatypeProperty rdf:about="http://example.org/onto/prop/google_colab_schedule_execution_user">
    <rdfs:label>execution_user</rdfs:label>
    <rdfs:comment>The user email to run the execution as.</rdfs:comment>
    <rdfs:domain rdf:resource="http://example.org/onto/class/google_colab_schedule"/>
    <rdfs:range rdf:resource="http://www.w3.org/2001/XMLSchema#string"/>
  </owl:DatatypeProperty>
  <owl:DatatypeProperty rdf:about="http://example.org/onto/prop/google_colab_schedule_gcs_output_uri">
    <rdfs:label>gcs_output_uri</rdfs:label>
    <rdfs:comment>The Cloud Storage location to upload the result to. Format:'gs://bucket-name'</rdfs:comment>
    <rdfs:domain rdf:resource="http://example.org/onto/class/google_colab_schedule"/>
    <rdfs:range rdf:resource="http://www.w3.org/2001/XMLSchema#string"/>
  </owl:DatatypeProperty>
  <owl:DatatypeProperty rdf:about="http://example.org/onto/prop/google_colab_schedule_notebook_runtime_template_resource_name">
    <rdfs:label>notebook_runtime_template_resource_name</rdfs:label>
    <rdfs:comment>The NotebookRuntimeTemplate to source compute configuration from.</rdfs:comment>
    <rdfs:domain rdf:resource="http://example.org/onto/class/google_colab_schedule"/>
    <rdfs:range rdf:resource="http://www.w3.org/2001/XMLSchema#string"/>
  </owl:DatatypeProperty>
  <owl:DatatypeProperty rdf:about="http://example.org/onto/prop/google_colab_schedule_service_account">
    <rdfs:label>service_account</rdfs:label>
    <rdfs:comment>The service account to run the execution as.</rdfs:comment>
    <rdfs:domain rdf:resource="http://example.org/onto/class/google_colab_schedule"/>
    <rdfs:range rdf:resource="http://www.w3.org/2001/XMLSchema#string"/>
  </owl:DatatypeProperty>
  <owl:DatatypeProperty rdf:about="http://example.org/onto/prop/google_colab_schedule_commit_sha">
    <rdfs:label>commit_sha</rdfs:label>
    <rdfs:comment>The commit SHA to read repository with. If unset, the file will be read at HEAD.</rdfs:comment>
    <rdfs:domain rdf:resource="http://example.org/onto/class/google_colab_schedule"/>
    <rdfs:range rdf:resource="http://www.w3.org/2001/XMLSchema#string"/>
  </owl:DatatypeProperty>
  <owl:DatatypeProperty rdf:about="http://example.org/onto/prop/google_colab_schedule_dataform_repository_resource_name">
    <rdfs:label>dataform_repository_resource_name</rdfs:label>
    <rdfs:comment>The resource name of the Dataform Repository.</rdfs:comment>
    <rdfs:domain rdf:resource="http://example.org/onto/class/google_colab_schedule"/>
    <rdfs:range rdf:resource="http://www.w3.org/2001/XMLSchema#string"/>
  </owl:DatatypeProperty>
  <owl:DatatypeProperty rdf:about="http://example.org/onto/prop/google_colab_schedule_generation">
    <rdfs:label>generation</rdfs:label>
    <rdfs:comment>The version of the Cloud Storage object to read. If unset, the current version of the object is read. See https://cloud.google.com/storage/docs/metadata#generation-number.</rdfs:comment>
    <rdfs:domain rdf:resource="http://example.org/onto/class/google_colab_schedule"/>
    <rdfs:range rdf:resource="http://www.w3.org/2001/XMLSchema#string"/>
  </owl:DatatypeProperty>
  <owl:DatatypeProperty rdf:about="http://example.org/onto/prop/google_colab_schedule_uri">
    <rdfs:label>uri</rdfs:label>
    <rdfs:comment>The Cloud Storage uri pointing to the ipynb file. Format: gs://bucket/notebook_file.ipynb</rdfs:comment>
    <rdfs:domain rdf:resource="http://example.org/onto/class/google_colab_schedule"/>
    <rdfs:range rdf:resource="http://www.w3.org/2001/XMLSchema#string"/>
  </owl:DatatypeProperty>
  <owl:DatatypeProperty rdf:about="http://example.org/onto/prop/google_colab_schedule_create">
    <rdfs:label>create</rdfs:label>
    <rdfs:domain rdf:resource="http://example.org/onto/class/google_colab_schedule"/>
    <rdfs:range rdf:resource="http://www.w3.org/2001/XMLSchema#string"/>
  </owl:DatatypeProperty>
  <owl:DatatypeProperty rdf:about="http://example.org/onto/prop/google_colab_schedule_delete">
    <rdfs:label>delete</rdfs:label>
    <rdfs:domain rdf:resource="http://example.org/onto/class/google_colab_schedule"/>
    <rdfs:range rdf:resource="http://www.w3.org/2001/XMLSchema#string"/>
  </owl:DatatypeProperty>
  <owl:DatatypeProperty rdf:about="http://example.org/onto/prop/google_colab_schedule_update">
    <rdfs:label>update</rdfs:label>
    <rdfs:domain rdf:resource="http://example.org/onto/class/google_colab_schedule"/>
    <rdfs:range rdf:resource="http://www.w3.org/2001/XMLSchema#string"/>
  </owl:DatatypeProperty>
</rdf:RDF>
