<?xml version="1.0" encoding="UTF-8"?>
<rdf:RDF
  xmlns:rdf="http://www.w3.org/1999/02/22-rdf-syntax-ns#"
  xmlns:rdfs="http://www.w3.org/2000/01/rdf-schema#"
  xmlns:owl="http://www.w3.org/2002/07/owl#"
  xmlns:xsd="http://www.w3.org/2001/XMLSchema#"
  xml:base="http://example.org/onto/">
  <owl:Class rdf:about="http://example.org/onto/class/google_sql_database">
    <rdfs:label>google_sql_database</rdfs:label>
    <rdfs:comment>#
#     ***     AUTO GENERATED CODE    ***    Type: MMv1     ***
#
# ----------------------------------------------------------------------------
#
#     This code is generated by Magic Modules using the following:
#
#     Configuration: https:#github.com/GoogleCloudPlatform/magic-modules/tree/main/mmv1/products/sql/Database.yaml
#     Template:      https:#github.com/GoogleCloudPlatform/magic-modules/tree/main/mmv1/templates/terraform/resource.html.markdown.tmpl
#
#     DO NOT EDIT this file directly. Any changes made to this file will be
#     overwritten during the next generation cycle.
#
# ----------------------------------------------------------------------------
subcategory: "Cloud SQL"
description: |-
  Represents a SQL database inside the Cloud SQL instance, hosted in
  Google's cloud.
---</rdfs:comment>
  </owl:Class>
  <owl:DatatypeProperty rdf:about="http://example.org/onto/prop/google_sql_database_charset">
    <rdfs:label>charset</rdfs:label>
    <rdfs:comment>The charset value. See MySQL's
[Supported Character Sets and Collations](https://dev.mysql.com/doc/refman/5.7/en/charset-charsets.html)
and Postgres' [Character Set Support](https://www.postgresql.org/docs/9.6/static/multibyte.html)
for more details and supported values. Postgres databases only support
a value of 'UTF8' at creation time.</rdfs:comment>
    <rdfs:domain rdf:resource="http://example.org/onto/class/google_sql_database"/>
    <rdfs:range rdf:resource="http://www.w3.org/2001/XMLSchema#string"/>
  </owl:DatatypeProperty>
  <owl:DatatypeProperty rdf:about="http://example.org/onto/prop/google_sql_database_collation">
    <rdfs:label>collation</rdfs:label>
    <rdfs:comment>The collation value. See MySQL's
[Supported Character Sets and Collations](https://dev.mysql.com/doc/refman/5.7/en/charset-charsets.html)
and Postgres' [Collation Support](https://www.postgresql.org/docs/9.6/static/collation.html)
for more details and supported values. Postgres databases only support
a value of 'en_US.UTF8' at creation time.</rdfs:comment>
    <rdfs:domain rdf:resource="http://example.org/onto/class/google_sql_database"/>
    <rdfs:range rdf:resource="http://www.w3.org/2001/XMLSchema#string"/>
  </owl:DatatypeProperty>
  <owl:DatatypeProperty rdf:about="http://example.org/onto/prop/google_sql_database_deletion_policy">
    <rdfs:label>deletion_policy</rdfs:label>
    <rdfs:comment>The deletion policy for the database. Setting ABANDON allows the resource
to be abandoned rather than deleted. This is useful for Postgres, where databases cannot be
deleted from the API if there are users other than cloudsqlsuperuser with access. Possible
values are: "ABANDON", "DELETE". Defaults to "DELETE".</rdfs:comment>
    <rdfs:domain rdf:resource="http://example.org/onto/class/google_sql_database"/>
    <rdfs:range rdf:resource="http://www.w3.org/2001/XMLSchema#string"/>
  </owl:DatatypeProperty>
  <owl:DatatypeProperty rdf:about="http://example.org/onto/prop/google_sql_database_id">
    <rdfs:label>id</rdfs:label>
    <rdfs:domain rdf:resource="http://example.org/onto/class/google_sql_database"/>
    <rdfs:range rdf:resource="http://www.w3.org/2001/XMLSchema#string"/>
  </owl:DatatypeProperty>
  <owl:DatatypeProperty rdf:about="http://example.org/onto/prop/google_sql_database_instance">
    <rdfs:label>instance</rdfs:label>
    <rdfs:comment>The name of the Cloud SQL instance. This does not include the project
ID.</rdfs:comment>
    <rdfs:domain rdf:resource="http://example.org/onto/class/google_sql_database"/>
    <rdfs:range rdf:resource="http://www.w3.org/2001/XMLSchema#string"/>
  </owl:DatatypeProperty>
  <owl:DatatypeProperty rdf:about="http://example.org/onto/prop/google_sql_database_name">
    <rdfs:label>name</rdfs:label>
    <rdfs:comment>The name of the database in the Cloud SQL instance.
This does not include the project ID or instance name.</rdfs:comment>
    <rdfs:domain rdf:resource="http://example.org/onto/class/google_sql_database"/>
    <rdfs:range rdf:resource="http://www.w3.org/2001/XMLSchema#string"/>
  </owl:DatatypeProperty>
  <owl:DatatypeProperty rdf:about="http://example.org/onto/prop/google_sql_database_project">
    <rdfs:label>project</rdfs:label>
    <rdfs:domain rdf:resource="http://example.org/onto/class/google_sql_database"/>
    <rdfs:range rdf:resource="http://www.w3.org/2001/XMLSchema#string"/>
  </owl:DatatypeProperty>
  <owl:DatatypeProperty rdf:about="http://example.org/onto/prop/google_sql_database_self_link">
    <rdfs:label>self_link</rdfs:label>
    <rdfs:domain rdf:resource="http://example.org/onto/class/google_sql_database"/>
    <rdfs:range rdf:resource="http://www.w3.org/2001/XMLSchema#string"/>
  </owl:DatatypeProperty>
  <owl:DatatypeProperty rdf:about="http://example.org/onto/prop/google_sql_database_create">
    <rdfs:label>create</rdfs:label>
    <rdfs:domain rdf:resource="http://example.org/onto/class/google_sql_database"/>
    <rdfs:range rdf:resource="http://www.w3.org/2001/XMLSchema#string"/>
  </owl:DatatypeProperty>
  <owl:DatatypeProperty rdf:about="http://example.org/onto/prop/google_sql_database_delete">
    <rdfs:label>delete</rdfs:label>
    <rdfs:domain rdf:resource="http://example.org/onto/class/google_sql_database"/>
    <rdfs:range rdf:resource="http://www.w3.org/2001/XMLSchema#string"/>
  </owl:DatatypeProperty>
  <owl:DatatypeProperty rdf:about="http://example.org/onto/prop/google_sql_database_update">
    <rdfs:label>update</rdfs:label>
    <rdfs:domain rdf:resource="http://example.org/onto/class/google_sql_database"/>
    <rdfs:range rdf:resource="http://www.w3.org/2001/XMLSchema#string"/>
  </owl:DatatypeProperty>
</rdf:RDF>
