<?xml version="1.0" encoding="UTF-8"?>
<rdf:RDF
  xmlns:rdf="http://www.w3.org/1999/02/22-rdf-syntax-ns#"
  xmlns:rdfs="http://www.w3.org/2000/01/rdf-schema#"
  xmlns:owl="http://www.w3.org/2002/07/owl#"
  xmlns:xsd="http://www.w3.org/2001/XMLSchema#"
  xml:base="http://example.org/onto/">
  <owl:Class rdf:about="http://example.org/onto/class/google_secret_manager_regional_secret">
    <rdfs:label>google_secret_manager_regional_secret</rdfs:label>
    <rdfs:comment>#
#     ***     AUTO GENERATED CODE    ***    Type: MMv1     ***
#
# ----------------------------------------------------------------------------
#
#     This code is generated by Magic Modules using the following:
#
#     Configuration: https:#github.com/GoogleCloudPlatform/magic-modules/tree/main/mmv1/products/secretmanagerregional/RegionalSecret.yaml
#     Template:      https:#github.com/GoogleCloudPlatform/magic-modules/tree/main/mmv1/templates/terraform/resource.html.markdown.tmpl
#
#     DO NOT EDIT this file directly. Any changes made to this file will be
#     overwritten during the next generation cycle.
#
# ----------------------------------------------------------------------------
subcategory: "Secret Manager"
description: |-
  A Regional Secret is a logical secret whose value and versions can be created and accessed within a region only.
---</rdfs:comment>
  </owl:Class>
  <owl:DatatypeProperty rdf:about="http://example.org/onto/prop/google_secret_manager_regional_secret_annotations">
    <rdfs:label>annotations</rdfs:label>
    <rdfs:comment>Custom metadata about the regional secret.

Annotations are distinct from various forms of labels. Annotations exist to allow
client tools to store their own state information without requiring a database.

Annotation keys must be between 1 and 63 characters long, have a UTF-8 encoding of
maximum 128 bytes, begin and end with an alphanumeric character ([a-z0-9A-Z]), and
may have dashes (-), underscores (_), dots (.), and alphanumerics in between these
symbols.

The total size of annotation keys and values must be less than 16KiB.

An object containing a list of "key": value pairs. Example:
{ "name": "wrench", "mass": "1.3kg", "count": "3" }.


**Note**: This field is non-authoritative, and will only manage the annotations present in your configuration.
Please refer to the field 'effective_annotations' for all of the annotations present on the resource.</rdfs:comment>
    <rdfs:domain rdf:resource="http://example.org/onto/class/google_secret_manager_regional_secret"/>
    <rdfs:range rdf:resource="http://www.w3.org/2001/XMLSchema#string"/>
  </owl:DatatypeProperty>
  <owl:DatatypeProperty rdf:about="http://example.org/onto/prop/google_secret_manager_regional_secret_create_time">
    <rdfs:label>create_time</rdfs:label>
    <rdfs:comment>The time at which the regional secret was created.</rdfs:comment>
    <rdfs:domain rdf:resource="http://example.org/onto/class/google_secret_manager_regional_secret"/>
    <rdfs:range rdf:resource="http://www.w3.org/2001/XMLSchema#string"/>
  </owl:DatatypeProperty>
  <owl:DatatypeProperty rdf:about="http://example.org/onto/prop/google_secret_manager_regional_secret_deletion_protection">
    <rdfs:label>deletion_protection</rdfs:label>
    <rdfs:comment>Whether Terraform will be prevented from destroying the regional secret. Defaults to false.
When the field is set to true in Terraform state, a 'terraform apply'
or 'terraform destroy' that would delete the federation will fail.</rdfs:comment>
    <rdfs:domain rdf:resource="http://example.org/onto/class/google_secret_manager_regional_secret"/>
    <rdfs:range rdf:resource="http://www.w3.org/2001/XMLSchema#string"/>
  </owl:DatatypeProperty>
  <owl:DatatypeProperty rdf:about="http://example.org/onto/prop/google_secret_manager_regional_secret_effective_annotations">
    <rdfs:label>effective_annotations</rdfs:label>
    <rdfs:comment>All of annotations (key/value pairs) present on the resource in GCP, including the annotations configured through Terraform, other clients and services.</rdfs:comment>
    <rdfs:domain rdf:resource="http://example.org/onto/class/google_secret_manager_regional_secret"/>
    <rdfs:range rdf:resource="http://www.w3.org/2001/XMLSchema#string"/>
  </owl:DatatypeProperty>
  <owl:DatatypeProperty rdf:about="http://example.org/onto/prop/google_secret_manager_regional_secret_effective_labels">
    <rdfs:label>effective_labels</rdfs:label>
    <rdfs:comment>All of labels (key/value pairs) present on the resource in GCP, including the labels configured through Terraform, other clients and services.</rdfs:comment>
    <rdfs:domain rdf:resource="http://example.org/onto/class/google_secret_manager_regional_secret"/>
    <rdfs:range rdf:resource="http://www.w3.org/2001/XMLSchema#string"/>
  </owl:DatatypeProperty>
  <owl:DatatypeProperty rdf:about="http://example.org/onto/prop/google_secret_manager_regional_secret_expire_time">
    <rdfs:label>expire_time</rdfs:label>
    <rdfs:comment>Timestamp in UTC when the regional secret is scheduled to expire. This is always provided on
output, regardless of what was sent on input. A timestamp in RFC3339 UTC "Zulu" format, with
nanosecond resolution and up to nine fractional digits. Examples: "2014-10-02T15:01:23Z" and
"2014-10-02T15:01:23.045123456Z". Only one of 'expire_time' or 'ttl' can be provided.</rdfs:comment>
    <rdfs:domain rdf:resource="http://example.org/onto/class/google_secret_manager_regional_secret"/>
    <rdfs:range rdf:resource="http://www.w3.org/2001/XMLSchema#string"/>
  </owl:DatatypeProperty>
  <owl:DatatypeProperty rdf:about="http://example.org/onto/prop/google_secret_manager_regional_secret_id">
    <rdfs:label>id</rdfs:label>
    <rdfs:domain rdf:resource="http://example.org/onto/class/google_secret_manager_regional_secret"/>
    <rdfs:range rdf:resource="http://www.w3.org/2001/XMLSchema#string"/>
  </owl:DatatypeProperty>
  <owl:DatatypeProperty rdf:about="http://example.org/onto/prop/google_secret_manager_regional_secret_labels">
    <rdfs:label>labels</rdfs:label>
    <rdfs:comment>The labels assigned to this regional secret.

Label keys must be between 1 and 63 characters long, have a UTF-8 encoding of maximum 128 bytes,
and must conform to the following PCRE regular expression: [\p{Ll}\p{Lo}][\p{Ll}\p{Lo}\p{N}_-]{0,62}

Label values must be between 0 and 63 characters long, have a UTF-8 encoding of maximum 128 bytes,
and must conform to the following PCRE regular expression: [\p{Ll}\p{Lo}\p{N}_-]{0,63}

No more than 64 labels can be assigned to a given resource.

An object containing a list of "key": value pairs. Example:
{ "name": "wrench", "mass": "1.3kg", "count": "3" }.


**Note**: This field is non-authoritative, and will only manage the labels present in your configuration.
Please refer to the field 'effective_labels' for all of the labels present on the resource.</rdfs:comment>
    <rdfs:domain rdf:resource="http://example.org/onto/class/google_secret_manager_regional_secret"/>
    <rdfs:range rdf:resource="http://www.w3.org/2001/XMLSchema#string"/>
  </owl:DatatypeProperty>
  <owl:DatatypeProperty rdf:about="http://example.org/onto/prop/google_secret_manager_regional_secret_location">
    <rdfs:label>location</rdfs:label>
    <rdfs:comment>The location of the regional secret. eg us-central1</rdfs:comment>
    <rdfs:domain rdf:resource="http://example.org/onto/class/google_secret_manager_regional_secret"/>
    <rdfs:range rdf:resource="http://www.w3.org/2001/XMLSchema#string"/>
  </owl:DatatypeProperty>
  <owl:DatatypeProperty rdf:about="http://example.org/onto/prop/google_secret_manager_regional_secret_name">
    <rdfs:label>name</rdfs:label>
    <rdfs:comment>The resource name of the regional secret. Format:
'projects/{{project}}/locations/{{location}}/secrets/{{secret_id}}'</rdfs:comment>
    <rdfs:domain rdf:resource="http://example.org/onto/class/google_secret_manager_regional_secret"/>
    <rdfs:range rdf:resource="http://www.w3.org/2001/XMLSchema#string"/>
  </owl:DatatypeProperty>
  <owl:DatatypeProperty rdf:about="http://example.org/onto/prop/google_secret_manager_regional_secret_project">
    <rdfs:label>project</rdfs:label>
    <rdfs:domain rdf:resource="http://example.org/onto/class/google_secret_manager_regional_secret"/>
    <rdfs:range rdf:resource="http://www.w3.org/2001/XMLSchema#string"/>
  </owl:DatatypeProperty>
  <owl:DatatypeProperty rdf:about="http://example.org/onto/prop/google_secret_manager_regional_secret_secret_id">
    <rdfs:label>secret_id</rdfs:label>
    <rdfs:comment>This must be unique within the project.</rdfs:comment>
    <rdfs:domain rdf:resource="http://example.org/onto/class/google_secret_manager_regional_secret"/>
    <rdfs:range rdf:resource="http://www.w3.org/2001/XMLSchema#string"/>
  </owl:DatatypeProperty>
  <owl:DatatypeProperty rdf:about="http://example.org/onto/prop/google_secret_manager_regional_secret_tags">
    <rdfs:label>tags</rdfs:label>
    <rdfs:comment>A map of resource manager tags.
Resource manager tag keys and values have the same definition as resource manager tags.
Keys must be in the format tagKeys/{tag_key_id}, and values are in the format tagValues/{tag_value_id}.</rdfs:comment>
    <rdfs:domain rdf:resource="http://example.org/onto/class/google_secret_manager_regional_secret"/>
    <rdfs:range rdf:resource="http://www.w3.org/2001/XMLSchema#string"/>
  </owl:DatatypeProperty>
  <owl:DatatypeProperty rdf:about="http://example.org/onto/prop/google_secret_manager_regional_secret_terraform_labels">
    <rdfs:label>terraform_labels</rdfs:label>
    <rdfs:comment>The combination of labels configured directly on the resource
 and default labels configured on the provider.</rdfs:comment>
    <rdfs:domain rdf:resource="http://example.org/onto/class/google_secret_manager_regional_secret"/>
    <rdfs:range rdf:resource="http://www.w3.org/2001/XMLSchema#string"/>
  </owl:DatatypeProperty>
  <owl:DatatypeProperty rdf:about="http://example.org/onto/prop/google_secret_manager_regional_secret_ttl">
    <rdfs:label>ttl</rdfs:label>
    <rdfs:comment>The TTL for the regional secret. A duration in seconds with up to nine fractional digits,
terminated by 's'. Example: "3.5s". Only one of 'ttl' or 'expire_time' can be provided.</rdfs:comment>
    <rdfs:domain rdf:resource="http://example.org/onto/class/google_secret_manager_regional_secret"/>
    <rdfs:range rdf:resource="http://www.w3.org/2001/XMLSchema#string"/>
  </owl:DatatypeProperty>
  <owl:DatatypeProperty rdf:about="http://example.org/onto/prop/google_secret_manager_regional_secret_version_aliases">
    <rdfs:label>version_aliases</rdfs:label>
    <rdfs:comment>Mapping from version alias to version name.

A version alias is a string with a maximum length of 63 characters and can contain
uppercase and lowercase letters, numerals, and the hyphen (-) and underscore ('_')
characters. An alias string must start with a letter and cannot be the string
'latest' or 'NEW'. No more than 50 aliases can be assigned to a given secret.

An object containing a list of "key": value pairs. Example:
{ "name": "wrench", "mass": "1.3kg", "count": "3" }.</rdfs:comment>
    <rdfs:domain rdf:resource="http://example.org/onto/class/google_secret_manager_regional_secret"/>
    <rdfs:range rdf:resource="http://www.w3.org/2001/XMLSchema#string"/>
  </owl:DatatypeProperty>
  <owl:DatatypeProperty rdf:about="http://example.org/onto/prop/google_secret_manager_regional_secret_version_destroy_ttl">
    <rdfs:label>version_destroy_ttl</rdfs:label>
    <rdfs:comment>Secret Version TTL after destruction request.
This is a part of the delayed delete feature on Secret Version.
For secret with versionDestroyTtl>0, version destruction doesn't happen immediately
on calling destroy instead the version goes to a disabled state and
the actual destruction happens after this TTL expires. It must be atleast 24h.</rdfs:comment>
    <rdfs:domain rdf:resource="http://example.org/onto/class/google_secret_manager_regional_secret"/>
    <rdfs:range rdf:resource="http://www.w3.org/2001/XMLSchema#string"/>
  </owl:DatatypeProperty>
  <owl:DatatypeProperty rdf:about="http://example.org/onto/prop/google_secret_manager_regional_secret_kms_key_name">
    <rdfs:label>kms_key_name</rdfs:label>
    <rdfs:comment>The resource name of the Cloud KMS CryptoKey used to encrypt secret payloads.</rdfs:comment>
    <rdfs:domain rdf:resource="http://example.org/onto/class/google_secret_manager_regional_secret"/>
    <rdfs:range rdf:resource="http://www.w3.org/2001/XMLSchema#string"/>
  </owl:DatatypeProperty>
  <owl:DatatypeProperty rdf:about="http://example.org/onto/prop/google_secret_manager_regional_secret_next_rotation_time">
    <rdfs:label>next_rotation_time</rdfs:label>
    <rdfs:comment>Timestamp in UTC at which the Secret is scheduled to rotate.
A timestamp in RFC3339 UTC "Zulu" format, with nanosecond resolution and up to nine
fractional digits. Examples: "2014-10-02T15:01:23Z" and "2014-10-02T15:01:23.045123456Z".</rdfs:comment>
    <rdfs:domain rdf:resource="http://example.org/onto/class/google_secret_manager_regional_secret"/>
    <rdfs:range rdf:resource="http://www.w3.org/2001/XMLSchema#string"/>
  </owl:DatatypeProperty>
  <owl:DatatypeProperty rdf:about="http://example.org/onto/prop/google_secret_manager_regional_secret_rotation_period">
    <rdfs:label>rotation_period</rdfs:label>
    <rdfs:comment>The Duration between rotation notifications. Must be in seconds and at least 3600s (1h)
and at most 3153600000s (100 years). If rotationPeriod is set, 'next_rotation_time' must
be set. 'next_rotation_time' will be advanced by this period when the service
automatically sends rotation notifications.</rdfs:comment>
    <rdfs:domain rdf:resource="http://example.org/onto/class/google_secret_manager_regional_secret"/>
    <rdfs:range rdf:resource="http://www.w3.org/2001/XMLSchema#string"/>
  </owl:DatatypeProperty>
  <owl:DatatypeProperty rdf:about="http://example.org/onto/prop/google_secret_manager_regional_secret_create">
    <rdfs:label>create</rdfs:label>
    <rdfs:domain rdf:resource="http://example.org/onto/class/google_secret_manager_regional_secret"/>
    <rdfs:range rdf:resource="http://www.w3.org/2001/XMLSchema#string"/>
  </owl:DatatypeProperty>
  <owl:DatatypeProperty rdf:about="http://example.org/onto/prop/google_secret_manager_regional_secret_delete">
    <rdfs:label>delete</rdfs:label>
    <rdfs:domain rdf:resource="http://example.org/onto/class/google_secret_manager_regional_secret"/>
    <rdfs:range rdf:resource="http://www.w3.org/2001/XMLSchema#string"/>
  </owl:DatatypeProperty>
  <owl:DatatypeProperty rdf:about="http://example.org/onto/prop/google_secret_manager_regional_secret_update">
    <rdfs:label>update</rdfs:label>
    <rdfs:domain rdf:resource="http://example.org/onto/class/google_secret_manager_regional_secret"/>
    <rdfs:range rdf:resource="http://www.w3.org/2001/XMLSchema#string"/>
  </owl:DatatypeProperty>
  <owl:DatatypeProperty rdf:about="http://example.org/onto/prop/google_secret_manager_regional_secret_name">
    <rdfs:label>name</rdfs:label>
    <rdfs:comment>The resource name of the Pub/Sub topic that will be published to, in the following format:
projects/*/topics/*. For publication to succeed, the Secret Manager Service
Agent service account must have pubsub.publisher permissions on the topic.</rdfs:comment>
    <rdfs:domain rdf:resource="http://example.org/onto/class/google_secret_manager_regional_secret"/>
    <rdfs:range rdf:resource="http://www.w3.org/2001/XMLSchema#string"/>
  </owl:DatatypeProperty>
</rdf:RDF>
