<?xml version="1.0" encoding="UTF-8"?>
<rdf:RDF
  xmlns:rdf="http://www.w3.org/1999/02/22-rdf-syntax-ns#"
  xmlns:rdfs="http://www.w3.org/2000/01/rdf-schema#"
  xmlns:owl="http://www.w3.org/2002/07/owl#"
  xmlns:xsd="http://www.w3.org/2001/XMLSchema#"
  xml:base="http://example.org/onto/">
  <owl:Class rdf:about="http://example.org/onto/class/google_dataproc_cluster">
    <rdfs:label>google_dataproc_cluster</rdfs:label>
    <rdfs:comment>#
#     ***     AUTO GENERATED CODE    ***    Type: Handwritten     ***
#
# ----------------------------------------------------------------------------
#
#     This code is generated by Magic Modules using the following:
#
#     Source file: https://github.com/GoogleCloudPlatform/magic-modules/tree/main/mmv1/third_party/terraform/website/docs/r/dataproc_cluster.html.markdown
#
#     DO NOT EDIT this file directly. Any changes made to this file will be
#     overwritten during the next generation cycle.
#
# ----------------------------------------------------------------------------
subcategory: "Dataproc"
description: |-
  Manages a Cloud Dataproc cluster resource.
---</rdfs:comment>
  </owl:Class>
  <owl:DatatypeProperty rdf:about="http://example.org/onto/prop/google_dataproc_cluster_effective_labels">
    <rdfs:label>effective_labels</rdfs:label>
    <rdfs:comment>All of labels (key/value pairs) present on the resource in GCP, including the labels configured through Terraform, other clients and services.</rdfs:comment>
    <rdfs:domain rdf:resource="http://example.org/onto/class/google_dataproc_cluster"/>
    <rdfs:range rdf:resource="http://www.w3.org/2001/XMLSchema#string"/>
  </owl:DatatypeProperty>
  <owl:DatatypeProperty rdf:about="http://example.org/onto/prop/google_dataproc_cluster_graceful_decommission_timeout">
    <rdfs:label>graceful_decommission_timeout</rdfs:label>
    <rdfs:comment>The timeout duration which allows graceful decomissioning when you change the number of worker nodes directly through a terraform apply</rdfs:comment>
    <rdfs:domain rdf:resource="http://example.org/onto/class/google_dataproc_cluster"/>
    <rdfs:range rdf:resource="http://www.w3.org/2001/XMLSchema#string"/>
  </owl:DatatypeProperty>
  <owl:DatatypeProperty rdf:about="http://example.org/onto/prop/google_dataproc_cluster_id">
    <rdfs:label>id</rdfs:label>
    <rdfs:domain rdf:resource="http://example.org/onto/class/google_dataproc_cluster"/>
    <rdfs:range rdf:resource="http://www.w3.org/2001/XMLSchema#string"/>
  </owl:DatatypeProperty>
  <owl:DatatypeProperty rdf:about="http://example.org/onto/prop/google_dataproc_cluster_labels">
    <rdfs:label>labels</rdfs:label>
    <rdfs:comment>The list of the labels (key/value pairs) configured on the resource and to be applied to instances in the cluster.

				**Note**: This field is non-authoritative, and will only manage the labels present in your configuration.
				Please refer to the field 'effective_labels' for all of the labels present on the resource.</rdfs:comment>
    <rdfs:domain rdf:resource="http://example.org/onto/class/google_dataproc_cluster"/>
    <rdfs:range rdf:resource="http://www.w3.org/2001/XMLSchema#string"/>
  </owl:DatatypeProperty>
  <owl:DatatypeProperty rdf:about="http://example.org/onto/prop/google_dataproc_cluster_name">
    <rdfs:label>name</rdfs:label>
    <rdfs:comment>The name of the cluster, unique within the project and zone.</rdfs:comment>
    <rdfs:domain rdf:resource="http://example.org/onto/class/google_dataproc_cluster"/>
    <rdfs:range rdf:resource="http://www.w3.org/2001/XMLSchema#string"/>
  </owl:DatatypeProperty>
  <owl:DatatypeProperty rdf:about="http://example.org/onto/prop/google_dataproc_cluster_project">
    <rdfs:label>project</rdfs:label>
    <rdfs:comment>The ID of the project in which the cluster will exist. If it is not provided, the provider project is used.</rdfs:comment>
    <rdfs:domain rdf:resource="http://example.org/onto/class/google_dataproc_cluster"/>
    <rdfs:range rdf:resource="http://www.w3.org/2001/XMLSchema#string"/>
  </owl:DatatypeProperty>
  <owl:DatatypeProperty rdf:about="http://example.org/onto/prop/google_dataproc_cluster_region">
    <rdfs:label>region</rdfs:label>
    <rdfs:comment>The region in which the cluster and associated nodes will be created in. Defaults to global.</rdfs:comment>
    <rdfs:domain rdf:resource="http://example.org/onto/class/google_dataproc_cluster"/>
    <rdfs:range rdf:resource="http://www.w3.org/2001/XMLSchema#string"/>
  </owl:DatatypeProperty>
  <owl:DatatypeProperty rdf:about="http://example.org/onto/prop/google_dataproc_cluster_terraform_labels">
    <rdfs:label>terraform_labels</rdfs:label>
    <rdfs:comment>The combination of labels configured directly on the resource and default labels configured on the provider.</rdfs:comment>
    <rdfs:domain rdf:resource="http://example.org/onto/class/google_dataproc_cluster"/>
    <rdfs:range rdf:resource="http://www.w3.org/2001/XMLSchema#string"/>
  </owl:DatatypeProperty>
  <owl:DatatypeProperty rdf:about="http://example.org/onto/prop/google_dataproc_cluster_bucket">
    <rdfs:label>bucket</rdfs:label>
    <rdfs:comment>The name of the cloud storage bucket ultimately used to house the staging data for the cluster. If staging_bucket is specified, it will contain this value, otherwise it will be the auto generated name.</rdfs:comment>
    <rdfs:domain rdf:resource="http://example.org/onto/class/google_dataproc_cluster"/>
    <rdfs:range rdf:resource="http://www.w3.org/2001/XMLSchema#string"/>
  </owl:DatatypeProperty>
  <owl:DatatypeProperty rdf:about="http://example.org/onto/prop/google_dataproc_cluster_cluster_tier">
    <rdfs:label>cluster_tier</rdfs:label>
    <rdfs:comment>Specifies the tier of the cluster created.</rdfs:comment>
    <rdfs:domain rdf:resource="http://example.org/onto/class/google_dataproc_cluster"/>
    <rdfs:range rdf:resource="http://www.w3.org/2001/XMLSchema#string"/>
  </owl:DatatypeProperty>
  <owl:DatatypeProperty rdf:about="http://example.org/onto/prop/google_dataproc_cluster_staging_bucket">
    <rdfs:label>staging_bucket</rdfs:label>
    <rdfs:comment>The Cloud Storage staging bucket used to stage files, such as Hadoop jars, between client machines and the cluster. Note: If you don't explicitly specify a staging_bucket then GCP will auto create / assign one for you. However, you are not guaranteed an auto generated bucket which is solely dedicated to your cluster; it may be shared with other clusters in the same region/zone also choosing to use the auto generation option.</rdfs:comment>
    <rdfs:domain rdf:resource="http://example.org/onto/class/google_dataproc_cluster"/>
    <rdfs:range rdf:resource="http://www.w3.org/2001/XMLSchema#string"/>
  </owl:DatatypeProperty>
  <owl:DatatypeProperty rdf:about="http://example.org/onto/prop/google_dataproc_cluster_temp_bucket">
    <rdfs:label>temp_bucket</rdfs:label>
    <rdfs:comment>The Cloud Storage temp bucket used to store ephemeral cluster and jobs data, such as Spark and MapReduce history files. Note: If you don't explicitly specify a temp_bucket then GCP will auto create / assign one for you.</rdfs:comment>
    <rdfs:domain rdf:resource="http://example.org/onto/class/google_dataproc_cluster"/>
    <rdfs:range rdf:resource="http://www.w3.org/2001/XMLSchema#string"/>
  </owl:DatatypeProperty>
  <owl:DatatypeProperty rdf:about="http://example.org/onto/prop/google_dataproc_cluster_policy_uri">
    <rdfs:label>policy_uri</rdfs:label>
    <rdfs:comment>The autoscaling policy used by the cluster.</rdfs:comment>
    <rdfs:domain rdf:resource="http://example.org/onto/class/google_dataproc_cluster"/>
    <rdfs:range rdf:resource="http://www.w3.org/2001/XMLSchema#string"/>
  </owl:DatatypeProperty>
  <owl:DatatypeProperty rdf:about="http://example.org/onto/prop/google_dataproc_cluster_node_group_id">
    <rdfs:label>node_group_id</rdfs:label>
    <rdfs:comment>A node group ID. Generated if not specified. The ID must contain only letters (a-z, A-Z), numbers (0-9), underscores (_), and hyphens (-). Cannot begin or end with underscore or hyphen. Must consist of from 3 to 33 characters.</rdfs:comment>
    <rdfs:domain rdf:resource="http://example.org/onto/class/google_dataproc_cluster"/>
    <rdfs:range rdf:resource="http://www.w3.org/2001/XMLSchema#string"/>
  </owl:DatatypeProperty>
  <owl:DatatypeProperty rdf:about="http://example.org/onto/prop/google_dataproc_cluster_name">
    <rdfs:label>name</rdfs:label>
    <rdfs:comment>The Node group resource name.</rdfs:comment>
    <rdfs:domain rdf:resource="http://example.org/onto/class/google_dataproc_cluster"/>
    <rdfs:range rdf:resource="http://www.w3.org/2001/XMLSchema#string"/>
  </owl:DatatypeProperty>
  <owl:DatatypeProperty rdf:about="http://example.org/onto/prop/google_dataproc_cluster_roles">
    <rdfs:label>roles</rdfs:label>
    <rdfs:comment>Node group roles.</rdfs:comment>
    <rdfs:domain rdf:resource="http://example.org/onto/class/google_dataproc_cluster"/>
    <rdfs:range rdf:resource="http://www.w3.org/2001/XMLSchema#string"/>
  </owl:DatatypeProperty>
  <owl:DatatypeProperty rdf:about="http://example.org/onto/prop/google_dataproc_cluster_instance_names">
    <rdfs:label>instance_names</rdfs:label>
    <rdfs:comment>List of auxiliary node group instance names which have been assigned to the cluster.</rdfs:comment>
    <rdfs:domain rdf:resource="http://example.org/onto/class/google_dataproc_cluster"/>
    <rdfs:range rdf:resource="http://www.w3.org/2001/XMLSchema#string"/>
  </owl:DatatypeProperty>
  <owl:DatatypeProperty rdf:about="http://example.org/onto/prop/google_dataproc_cluster_machine_type">
    <rdfs:label>machine_type</rdfs:label>
    <rdfs:comment>The name of a Google Compute Engine machine type to create for the master</rdfs:comment>
    <rdfs:domain rdf:resource="http://example.org/onto/class/google_dataproc_cluster"/>
    <rdfs:range rdf:resource="http://www.w3.org/2001/XMLSchema#string"/>
  </owl:DatatypeProperty>
  <owl:DatatypeProperty rdf:about="http://example.org/onto/prop/google_dataproc_cluster_min_cpu_platform">
    <rdfs:label>min_cpu_platform</rdfs:label>
    <rdfs:comment>The name of a minimum generation of CPU family for the auxiliary node group. If not specified, GCP will default to a predetermined computed value for each zone.</rdfs:comment>
    <rdfs:domain rdf:resource="http://example.org/onto/class/google_dataproc_cluster"/>
    <rdfs:range rdf:resource="http://www.w3.org/2001/XMLSchema#string"/>
  </owl:DatatypeProperty>
  <owl:DatatypeProperty rdf:about="http://example.org/onto/prop/google_dataproc_cluster_num_instances">
    <rdfs:label>num_instances</rdfs:label>
    <rdfs:comment>Specifies the number of auxiliary nodes to create. If not specified, GCP will default to a predetermined computed value.</rdfs:comment>
    <rdfs:domain rdf:resource="http://example.org/onto/class/google_dataproc_cluster"/>
    <rdfs:range rdf:resource="http://www.w3.org/2001/XMLSchema#string"/>
  </owl:DatatypeProperty>
  <owl:DatatypeProperty rdf:about="http://example.org/onto/prop/google_dataproc_cluster_accelerator_count">
    <rdfs:label>accelerator_count</rdfs:label>
    <rdfs:comment>The number of the accelerator cards of this type exposed to this instance. Often restricted to one of 1, 2, 4, or 8.</rdfs:comment>
    <rdfs:domain rdf:resource="http://example.org/onto/class/google_dataproc_cluster"/>
    <rdfs:range rdf:resource="http://www.w3.org/2001/XMLSchema#string"/>
  </owl:DatatypeProperty>
  <owl:DatatypeProperty rdf:about="http://example.org/onto/prop/google_dataproc_cluster_accelerator_type">
    <rdfs:label>accelerator_type</rdfs:label>
    <rdfs:comment>The short name of the accelerator type to expose to this instance. For example, nvidia-tesla-k80.</rdfs:comment>
    <rdfs:domain rdf:resource="http://example.org/onto/class/google_dataproc_cluster"/>
    <rdfs:range rdf:resource="http://www.w3.org/2001/XMLSchema#string"/>
  </owl:DatatypeProperty>
  <owl:DatatypeProperty rdf:about="http://example.org/onto/prop/google_dataproc_cluster_boot_disk_size_gb">
    <rdfs:label>boot_disk_size_gb</rdfs:label>
    <rdfs:comment>Size of the primary disk attached to each node, specified in GB. The primary disk contains the boot volume and system libraries, and the smallest allowed disk size is 10GB. GCP will default to a predetermined computed value if not set (currently 500GB). Note: If SSDs are not attached, it also contains the HDFS data blocks and Hadoop working directories.</rdfs:comment>
    <rdfs:domain rdf:resource="http://example.org/onto/class/google_dataproc_cluster"/>
    <rdfs:range rdf:resource="http://www.w3.org/2001/XMLSchema#string"/>
  </owl:DatatypeProperty>
  <owl:DatatypeProperty rdf:about="http://example.org/onto/prop/google_dataproc_cluster_boot_disk_type">
    <rdfs:label>boot_disk_type</rdfs:label>
    <rdfs:comment>The disk type of the primary disk attached to each node. Such as "pd-ssd" or "pd-standard". Defaults to "pd-standard".</rdfs:comment>
    <rdfs:domain rdf:resource="http://example.org/onto/class/google_dataproc_cluster"/>
    <rdfs:range rdf:resource="http://www.w3.org/2001/XMLSchema#string"/>
  </owl:DatatypeProperty>
  <owl:DatatypeProperty rdf:about="http://example.org/onto/prop/google_dataproc_cluster_local_ssd_interface">
    <rdfs:label>local_ssd_interface</rdfs:label>
    <rdfs:comment>Interface type of local SSDs (default is "scsi"). Valid values: "scsi" (Small Computer System Interface), "nvme" (Non-Volatile Memory Express).</rdfs:comment>
    <rdfs:domain rdf:resource="http://example.org/onto/class/google_dataproc_cluster"/>
    <rdfs:range rdf:resource="http://www.w3.org/2001/XMLSchema#string"/>
  </owl:DatatypeProperty>
  <owl:DatatypeProperty rdf:about="http://example.org/onto/prop/google_dataproc_cluster_num_local_ssds">
    <rdfs:label>num_local_ssds</rdfs:label>
    <rdfs:comment>The amount of local SSD disks that will be attached to each master cluster node. Defaults to 0.</rdfs:comment>
    <rdfs:domain rdf:resource="http://example.org/onto/class/google_dataproc_cluster"/>
    <rdfs:range rdf:resource="http://www.w3.org/2001/XMLSchema#string"/>
  </owl:DatatypeProperty>
  <owl:DatatypeProperty rdf:about="http://example.org/onto/prop/google_dataproc_cluster_metric_overrides">
    <rdfs:label>metric_overrides</rdfs:label>
    <rdfs:comment>Specify one or more [available OSS metrics] (https://cloud.google.com/dataproc/docs/guides/monitoring#available_oss_metrics) to collect.</rdfs:comment>
    <rdfs:domain rdf:resource="http://example.org/onto/class/google_dataproc_cluster"/>
    <rdfs:range rdf:resource="http://www.w3.org/2001/XMLSchema#string"/>
  </owl:DatatypeProperty>
  <owl:DatatypeProperty rdf:about="http://example.org/onto/prop/google_dataproc_cluster_metric_source">
    <rdfs:label>metric_source</rdfs:label>
    <rdfs:comment>A source for the collection of Dataproc OSS metrics (see [available OSS metrics] (https://cloud.google.com//dataproc/docs/guides/monitoring#available_oss_metrics)).</rdfs:comment>
    <rdfs:domain rdf:resource="http://example.org/onto/class/google_dataproc_cluster"/>
    <rdfs:range rdf:resource="http://www.w3.org/2001/XMLSchema#string"/>
  </owl:DatatypeProperty>
  <owl:DatatypeProperty rdf:about="http://example.org/onto/prop/google_dataproc_cluster_kms_key_name">
    <rdfs:label>kms_key_name</rdfs:label>
    <rdfs:comment>The Cloud KMS key name to use for PD disk encryption for all instances in the cluster.</rdfs:comment>
    <rdfs:domain rdf:resource="http://example.org/onto/class/google_dataproc_cluster"/>
    <rdfs:range rdf:resource="http://www.w3.org/2001/XMLSchema#string"/>
  </owl:DatatypeProperty>
  <owl:DatatypeProperty rdf:about="http://example.org/onto/prop/google_dataproc_cluster_enable_http_port_access">
    <rdfs:label>enable_http_port_access</rdfs:label>
    <rdfs:comment>The flag to enable http access to specific ports on the cluster from external sources (aka Component Gateway). Defaults to false.</rdfs:comment>
    <rdfs:domain rdf:resource="http://example.org/onto/class/google_dataproc_cluster"/>
    <rdfs:range rdf:resource="http://www.w3.org/2001/XMLSchema#string"/>
  </owl:DatatypeProperty>
  <owl:DatatypeProperty rdf:about="http://example.org/onto/prop/google_dataproc_cluster_http_ports">
    <rdfs:label>http_ports</rdfs:label>
    <rdfs:comment>The map of port descriptions to URLs. Will only be populated if enable_http_port_access is true.</rdfs:comment>
    <rdfs:domain rdf:resource="http://example.org/onto/class/google_dataproc_cluster"/>
    <rdfs:range rdf:resource="http://www.w3.org/2001/XMLSchema#string"/>
  </owl:DatatypeProperty>
  <owl:DatatypeProperty rdf:about="http://example.org/onto/prop/google_dataproc_cluster_internal_ip_only">
    <rdfs:label>internal_ip_only</rdfs:label>
    <rdfs:comment>By default, clusters are not restricted to internal IP addresses, and will have ephemeral external IP addresses assigned to each instance. If set to true, all instances in the cluster will only have internal IP addresses. Note: Private Google Access (also known as privateIpGoogleAccess) must be enabled on the subnetwork that the cluster will be launched in.</rdfs:comment>
    <rdfs:domain rdf:resource="http://example.org/onto/class/google_dataproc_cluster"/>
    <rdfs:range rdf:resource="http://www.w3.org/2001/XMLSchema#string"/>
  </owl:DatatypeProperty>
  <owl:DatatypeProperty rdf:about="http://example.org/onto/prop/google_dataproc_cluster_metadata">
    <rdfs:label>metadata</rdfs:label>
    <rdfs:comment>A map of the Compute Engine metadata entries to add to all instances</rdfs:comment>
    <rdfs:domain rdf:resource="http://example.org/onto/class/google_dataproc_cluster"/>
    <rdfs:range rdf:resource="http://www.w3.org/2001/XMLSchema#string"/>
  </owl:DatatypeProperty>
  <owl:DatatypeProperty rdf:about="http://example.org/onto/prop/google_dataproc_cluster_network">
    <rdfs:label>network</rdfs:label>
    <rdfs:comment>The name or self_link of the Google Compute Engine network to the cluster will be part of. Conflicts with subnetwork. If neither is specified, this defaults to the "default" network.</rdfs:comment>
    <rdfs:domain rdf:resource="http://example.org/onto/class/google_dataproc_cluster"/>
    <rdfs:range rdf:resource="http://www.w3.org/2001/XMLSchema#string"/>
  </owl:DatatypeProperty>
  <owl:DatatypeProperty rdf:about="http://example.org/onto/prop/google_dataproc_cluster_service_account">
    <rdfs:label>service_account</rdfs:label>
    <rdfs:comment>The service account to be used by the Node VMs. If not specified, the "default" service account is used.</rdfs:comment>
    <rdfs:domain rdf:resource="http://example.org/onto/class/google_dataproc_cluster"/>
    <rdfs:range rdf:resource="http://www.w3.org/2001/XMLSchema#string"/>
  </owl:DatatypeProperty>
  <owl:DatatypeProperty rdf:about="http://example.org/onto/prop/google_dataproc_cluster_service_account_scopes">
    <rdfs:label>service_account_scopes</rdfs:label>
    <rdfs:comment>The set of Google API scopes to be made available on all of the node VMs under the service_account specified. These can be either FQDNs, or scope aliases.</rdfs:comment>
    <rdfs:domain rdf:resource="http://example.org/onto/class/google_dataproc_cluster"/>
    <rdfs:range rdf:resource="http://www.w3.org/2001/XMLSchema#string"/>
  </owl:DatatypeProperty>
  <owl:DatatypeProperty rdf:about="http://example.org/onto/prop/google_dataproc_cluster_subnetwork">
    <rdfs:label>subnetwork</rdfs:label>
    <rdfs:comment>The name or self_link of the Google Compute Engine subnetwork the cluster will be part of. Conflicts with network.</rdfs:comment>
    <rdfs:domain rdf:resource="http://example.org/onto/class/google_dataproc_cluster"/>
    <rdfs:range rdf:resource="http://www.w3.org/2001/XMLSchema#string"/>
  </owl:DatatypeProperty>
  <owl:DatatypeProperty rdf:about="http://example.org/onto/prop/google_dataproc_cluster_tags">
    <rdfs:label>tags</rdfs:label>
    <rdfs:comment>The list of instance tags applied to instances in the cluster. Tags are used to identify valid sources or targets for network firewalls.</rdfs:comment>
    <rdfs:domain rdf:resource="http://example.org/onto/class/google_dataproc_cluster"/>
    <rdfs:range rdf:resource="http://www.w3.org/2001/XMLSchema#string"/>
  </owl:DatatypeProperty>
  <owl:DatatypeProperty rdf:about="http://example.org/onto/prop/google_dataproc_cluster_zone">
    <rdfs:label>zone</rdfs:label>
    <rdfs:comment>The GCP zone where your data is stored and used (i.e. where the master and the worker nodes will be created in). If region is set to 'global' (default) then zone is mandatory, otherwise GCP is able to make use of Auto Zone Placement to determine this automatically for you. Note: This setting additionally determines and restricts which computing resources are available for use with other configs such as cluster_config.master_config.machine_type and cluster_config.worker_config.machine_type.</rdfs:comment>
    <rdfs:domain rdf:resource="http://example.org/onto/class/google_dataproc_cluster"/>
    <rdfs:range rdf:resource="http://www.w3.org/2001/XMLSchema#string"/>
  </owl:DatatypeProperty>
  <owl:DatatypeProperty rdf:about="http://example.org/onto/prop/google_dataproc_cluster_enable_confidential_compute">
    <rdfs:label>enable_confidential_compute</rdfs:label>
    <rdfs:comment>Defines whether the instance should have confidential compute enabled.</rdfs:comment>
    <rdfs:domain rdf:resource="http://example.org/onto/class/google_dataproc_cluster"/>
    <rdfs:range rdf:resource="http://www.w3.org/2001/XMLSchema#string"/>
  </owl:DatatypeProperty>
  <owl:DatatypeProperty rdf:about="http://example.org/onto/prop/google_dataproc_cluster_node_group_uri">
    <rdfs:label>node_group_uri</rdfs:label>
    <rdfs:comment>The URI of a sole-tenant that the cluster will be created on.</rdfs:comment>
    <rdfs:domain rdf:resource="http://example.org/onto/class/google_dataproc_cluster"/>
    <rdfs:range rdf:resource="http://www.w3.org/2001/XMLSchema#string"/>
  </owl:DatatypeProperty>
  <owl:DatatypeProperty rdf:about="http://example.org/onto/prop/google_dataproc_cluster_consume_reservation_type">
    <rdfs:label>consume_reservation_type</rdfs:label>
    <rdfs:comment>Type of reservation to consume.</rdfs:comment>
    <rdfs:domain rdf:resource="http://example.org/onto/class/google_dataproc_cluster"/>
    <rdfs:range rdf:resource="http://www.w3.org/2001/XMLSchema#string"/>
  </owl:DatatypeProperty>
  <owl:DatatypeProperty rdf:about="http://example.org/onto/prop/google_dataproc_cluster_key">
    <rdfs:label>key</rdfs:label>
    <rdfs:comment>Corresponds to the label key of reservation resource.</rdfs:comment>
    <rdfs:domain rdf:resource="http://example.org/onto/class/google_dataproc_cluster"/>
    <rdfs:range rdf:resource="http://www.w3.org/2001/XMLSchema#string"/>
  </owl:DatatypeProperty>
  <owl:DatatypeProperty rdf:about="http://example.org/onto/prop/google_dataproc_cluster_values">
    <rdfs:label>values</rdfs:label>
    <rdfs:comment>Corresponds to the label values of reservation resource.</rdfs:comment>
    <rdfs:domain rdf:resource="http://example.org/onto/class/google_dataproc_cluster"/>
    <rdfs:range rdf:resource="http://www.w3.org/2001/XMLSchema#string"/>
  </owl:DatatypeProperty>
  <owl:DatatypeProperty rdf:about="http://example.org/onto/prop/google_dataproc_cluster_enable_integrity_monitoring">
    <rdfs:label>enable_integrity_monitoring</rdfs:label>
    <rdfs:comment>Defines whether instances have integrity monitoring enabled.</rdfs:comment>
    <rdfs:domain rdf:resource="http://example.org/onto/class/google_dataproc_cluster"/>
    <rdfs:range rdf:resource="http://www.w3.org/2001/XMLSchema#string"/>
  </owl:DatatypeProperty>
  <owl:DatatypeProperty rdf:about="http://example.org/onto/prop/google_dataproc_cluster_enable_secure_boot">
    <rdfs:label>enable_secure_boot</rdfs:label>
    <rdfs:comment>Defines whether instances have Secure Boot enabled.</rdfs:comment>
    <rdfs:domain rdf:resource="http://example.org/onto/class/google_dataproc_cluster"/>
    <rdfs:range rdf:resource="http://www.w3.org/2001/XMLSchema#string"/>
  </owl:DatatypeProperty>
  <owl:DatatypeProperty rdf:about="http://example.org/onto/prop/google_dataproc_cluster_enable_vtpm">
    <rdfs:label>enable_vtpm</rdfs:label>
    <rdfs:comment>Defines whether instances have the vTPM enabled.</rdfs:comment>
    <rdfs:domain rdf:resource="http://example.org/onto/class/google_dataproc_cluster"/>
    <rdfs:range rdf:resource="http://www.w3.org/2001/XMLSchema#string"/>
  </owl:DatatypeProperty>
  <owl:DatatypeProperty rdf:about="http://example.org/onto/prop/google_dataproc_cluster_script">
    <rdfs:label>script</rdfs:label>
    <rdfs:comment>The script to be executed during initialization of the cluster. The script must be a GCS file with a gs:// prefix.</rdfs:comment>
    <rdfs:domain rdf:resource="http://example.org/onto/class/google_dataproc_cluster"/>
    <rdfs:range rdf:resource="http://www.w3.org/2001/XMLSchema#string"/>
  </owl:DatatypeProperty>
  <owl:DatatypeProperty rdf:about="http://example.org/onto/prop/google_dataproc_cluster_timeout_sec">
    <rdfs:label>timeout_sec</rdfs:label>
    <rdfs:comment>The maximum duration (in seconds) which script is allowed to take to execute its action. GCP will default to a predetermined computed value if not set (currently 300).</rdfs:comment>
    <rdfs:domain rdf:resource="http://example.org/onto/class/google_dataproc_cluster"/>
    <rdfs:range rdf:resource="http://www.w3.org/2001/XMLSchema#string"/>
  </owl:DatatypeProperty>
  <owl:DatatypeProperty rdf:about="http://example.org/onto/prop/google_dataproc_cluster_auto_delete_time">
    <rdfs:label>auto_delete_time</rdfs:label>
    <rdfs:comment>The time when cluster will be auto-deleted. A timestamp in RFC3339 UTC "Zulu" format, accurate to nanoseconds. Example: "2014-10-02T15:01:23.045123456Z".</rdfs:comment>
    <rdfs:domain rdf:resource="http://example.org/onto/class/google_dataproc_cluster"/>
    <rdfs:range rdf:resource="http://www.w3.org/2001/XMLSchema#string"/>
  </owl:DatatypeProperty>
  <owl:DatatypeProperty rdf:about="http://example.org/onto/prop/google_dataproc_cluster_idle_delete_ttl">
    <rdfs:label>idle_delete_ttl</rdfs:label>
    <rdfs:comment>The duration to keep the cluster alive while idling (no jobs running). After this TTL, the cluster will be deleted. Valid range: [10m, 14d].</rdfs:comment>
    <rdfs:domain rdf:resource="http://example.org/onto/class/google_dataproc_cluster"/>
    <rdfs:range rdf:resource="http://www.w3.org/2001/XMLSchema#string"/>
  </owl:DatatypeProperty>
  <owl:DatatypeProperty rdf:about="http://example.org/onto/prop/google_dataproc_cluster_idle_start_time">
    <rdfs:label>idle_start_time</rdfs:label>
    <rdfs:comment>Time when the cluster became idle (most recent job finished) and became eligible for deletion due to idleness.</rdfs:comment>
    <rdfs:domain rdf:resource="http://example.org/onto/class/google_dataproc_cluster"/>
    <rdfs:range rdf:resource="http://www.w3.org/2001/XMLSchema#string"/>
  </owl:DatatypeProperty>
  <owl:DatatypeProperty rdf:about="http://example.org/onto/prop/google_dataproc_cluster_image_uri">
    <rdfs:label>image_uri</rdfs:label>
    <rdfs:comment>The URI for the image to use for this master</rdfs:comment>
    <rdfs:domain rdf:resource="http://example.org/onto/class/google_dataproc_cluster"/>
    <rdfs:range rdf:resource="http://www.w3.org/2001/XMLSchema#string"/>
  </owl:DatatypeProperty>
  <owl:DatatypeProperty rdf:about="http://example.org/onto/prop/google_dataproc_cluster_instance_names">
    <rdfs:label>instance_names</rdfs:label>
    <rdfs:comment>List of master instance names which have been assigned to the cluster.</rdfs:comment>
    <rdfs:domain rdf:resource="http://example.org/onto/class/google_dataproc_cluster"/>
    <rdfs:range rdf:resource="http://www.w3.org/2001/XMLSchema#string"/>
  </owl:DatatypeProperty>
  <owl:DatatypeProperty rdf:about="http://example.org/onto/prop/google_dataproc_cluster_machine_type">
    <rdfs:label>machine_type</rdfs:label>
    <rdfs:comment>The name of a Google Compute Engine machine type to create for the master</rdfs:comment>
    <rdfs:domain rdf:resource="http://example.org/onto/class/google_dataproc_cluster"/>
    <rdfs:range rdf:resource="http://www.w3.org/2001/XMLSchema#string"/>
  </owl:DatatypeProperty>
  <owl:DatatypeProperty rdf:about="http://example.org/onto/prop/google_dataproc_cluster_min_cpu_platform">
    <rdfs:label>min_cpu_platform</rdfs:label>
    <rdfs:comment>The name of a minimum generation of CPU family for the master. If not specified, GCP will default to a predetermined computed value for each zone.</rdfs:comment>
    <rdfs:domain rdf:resource="http://example.org/onto/class/google_dataproc_cluster"/>
    <rdfs:range rdf:resource="http://www.w3.org/2001/XMLSchema#string"/>
  </owl:DatatypeProperty>
  <owl:DatatypeProperty rdf:about="http://example.org/onto/prop/google_dataproc_cluster_num_instances">
    <rdfs:label>num_instances</rdfs:label>
    <rdfs:comment>Specifies the number of master nodes to create. If not specified, GCP will default to a predetermined computed value.</rdfs:comment>
    <rdfs:domain rdf:resource="http://example.org/onto/class/google_dataproc_cluster"/>
    <rdfs:range rdf:resource="http://www.w3.org/2001/XMLSchema#string"/>
  </owl:DatatypeProperty>
  <owl:DatatypeProperty rdf:about="http://example.org/onto/prop/google_dataproc_cluster_accelerator_count">
    <rdfs:label>accelerator_count</rdfs:label>
    <rdfs:comment>The number of the accelerator cards of this type exposed to this instance. Often restricted to one of 1, 2, 4, or 8.</rdfs:comment>
    <rdfs:domain rdf:resource="http://example.org/onto/class/google_dataproc_cluster"/>
    <rdfs:range rdf:resource="http://www.w3.org/2001/XMLSchema#string"/>
  </owl:DatatypeProperty>
  <owl:DatatypeProperty rdf:about="http://example.org/onto/prop/google_dataproc_cluster_accelerator_type">
    <rdfs:label>accelerator_type</rdfs:label>
    <rdfs:comment>The short name of the accelerator type to expose to this instance. For example, nvidia-tesla-k80.</rdfs:comment>
    <rdfs:domain rdf:resource="http://example.org/onto/class/google_dataproc_cluster"/>
    <rdfs:range rdf:resource="http://www.w3.org/2001/XMLSchema#string"/>
  </owl:DatatypeProperty>
  <owl:DatatypeProperty rdf:about="http://example.org/onto/prop/google_dataproc_cluster_boot_disk_size_gb">
    <rdfs:label>boot_disk_size_gb</rdfs:label>
    <rdfs:comment>Size of the primary disk attached to each node, specified in GB. The primary disk contains the boot volume and system libraries, and the smallest allowed disk size is 10GB. GCP will default to a predetermined computed value if not set (currently 500GB). Note: If SSDs are not attached, it also contains the HDFS data blocks and Hadoop working directories.</rdfs:comment>
    <rdfs:domain rdf:resource="http://example.org/onto/class/google_dataproc_cluster"/>
    <rdfs:range rdf:resource="http://www.w3.org/2001/XMLSchema#string"/>
  </owl:DatatypeProperty>
  <owl:DatatypeProperty rdf:about="http://example.org/onto/prop/google_dataproc_cluster_boot_disk_type">
    <rdfs:label>boot_disk_type</rdfs:label>
    <rdfs:comment>The disk type of the primary disk attached to each node. Such as "pd-ssd" or "pd-standard". Defaults to "pd-standard".</rdfs:comment>
    <rdfs:domain rdf:resource="http://example.org/onto/class/google_dataproc_cluster"/>
    <rdfs:range rdf:resource="http://www.w3.org/2001/XMLSchema#string"/>
  </owl:DatatypeProperty>
  <owl:DatatypeProperty rdf:about="http://example.org/onto/prop/google_dataproc_cluster_local_ssd_interface">
    <rdfs:label>local_ssd_interface</rdfs:label>
    <rdfs:comment>Interface type of local SSDs (default is "scsi"). Valid values: "scsi" (Small Computer System Interface), "nvme" (Non-Volatile Memory Express).</rdfs:comment>
    <rdfs:domain rdf:resource="http://example.org/onto/class/google_dataproc_cluster"/>
    <rdfs:range rdf:resource="http://www.w3.org/2001/XMLSchema#string"/>
  </owl:DatatypeProperty>
  <owl:DatatypeProperty rdf:about="http://example.org/onto/prop/google_dataproc_cluster_num_local_ssds">
    <rdfs:label>num_local_ssds</rdfs:label>
    <rdfs:comment>The amount of local SSD disks that will be attached to each master cluster node. Defaults to 0.</rdfs:comment>
    <rdfs:domain rdf:resource="http://example.org/onto/class/google_dataproc_cluster"/>
    <rdfs:range rdf:resource="http://www.w3.org/2001/XMLSchema#string"/>
  </owl:DatatypeProperty>
  <owl:DatatypeProperty rdf:about="http://example.org/onto/prop/google_dataproc_cluster_dataproc_metastore_service">
    <rdfs:label>dataproc_metastore_service</rdfs:label>
    <rdfs:comment>Resource name of an existing Dataproc Metastore service.</rdfs:comment>
    <rdfs:domain rdf:resource="http://example.org/onto/class/google_dataproc_cluster"/>
    <rdfs:range rdf:resource="http://www.w3.org/2001/XMLSchema#string"/>
  </owl:DatatypeProperty>
  <owl:DatatypeProperty rdf:about="http://example.org/onto/prop/google_dataproc_cluster_instance_names">
    <rdfs:label>instance_names</rdfs:label>
    <rdfs:comment>List of preemptible instance names which have been assigned to the cluster.</rdfs:comment>
    <rdfs:domain rdf:resource="http://example.org/onto/class/google_dataproc_cluster"/>
    <rdfs:range rdf:resource="http://www.w3.org/2001/XMLSchema#string"/>
  </owl:DatatypeProperty>
  <owl:DatatypeProperty rdf:about="http://example.org/onto/prop/google_dataproc_cluster_num_instances">
    <rdfs:label>num_instances</rdfs:label>
    <rdfs:comment>Specifies the number of preemptible nodes to create. Defaults to 0.</rdfs:comment>
    <rdfs:domain rdf:resource="http://example.org/onto/class/google_dataproc_cluster"/>
    <rdfs:range rdf:resource="http://www.w3.org/2001/XMLSchema#string"/>
  </owl:DatatypeProperty>
  <owl:DatatypeProperty rdf:about="http://example.org/onto/prop/google_dataproc_cluster_preemptibility">
    <rdfs:label>preemptibility</rdfs:label>
    <rdfs:comment>Specifies the preemptibility of the secondary nodes. Defaults to PREEMPTIBLE.</rdfs:comment>
    <rdfs:domain rdf:resource="http://example.org/onto/class/google_dataproc_cluster"/>
    <rdfs:range rdf:resource="http://www.w3.org/2001/XMLSchema#string"/>
  </owl:DatatypeProperty>
  <owl:DatatypeProperty rdf:about="http://example.org/onto/prop/google_dataproc_cluster_boot_disk_size_gb">
    <rdfs:label>boot_disk_size_gb</rdfs:label>
    <rdfs:comment>Size of the primary disk attached to each preemptible worker node, specified in GB. The smallest allowed disk size is 10GB. GCP will default to a predetermined computed value if not set (currently 500GB). Note: If SSDs are not attached, it also contains the HDFS data blocks and Hadoop working directories.</rdfs:comment>
    <rdfs:domain rdf:resource="http://example.org/onto/class/google_dataproc_cluster"/>
    <rdfs:range rdf:resource="http://www.w3.org/2001/XMLSchema#string"/>
  </owl:DatatypeProperty>
  <owl:DatatypeProperty rdf:about="http://example.org/onto/prop/google_dataproc_cluster_boot_disk_type">
    <rdfs:label>boot_disk_type</rdfs:label>
    <rdfs:comment>The disk type of the primary disk attached to each preemptible worker node. Such as "pd-ssd" or "pd-standard". Defaults to "pd-standard".</rdfs:comment>
    <rdfs:domain rdf:resource="http://example.org/onto/class/google_dataproc_cluster"/>
    <rdfs:range rdf:resource="http://www.w3.org/2001/XMLSchema#string"/>
  </owl:DatatypeProperty>
  <owl:DatatypeProperty rdf:about="http://example.org/onto/prop/google_dataproc_cluster_local_ssd_interface">
    <rdfs:label>local_ssd_interface</rdfs:label>
    <rdfs:comment>Interface type of local SSDs (default is "scsi"). Valid values: "scsi" (Small Computer System Interface), "nvme" (Non-Volatile Memory Express).</rdfs:comment>
    <rdfs:domain rdf:resource="http://example.org/onto/class/google_dataproc_cluster"/>
    <rdfs:range rdf:resource="http://www.w3.org/2001/XMLSchema#string"/>
  </owl:DatatypeProperty>
  <owl:DatatypeProperty rdf:about="http://example.org/onto/prop/google_dataproc_cluster_num_local_ssds">
    <rdfs:label>num_local_ssds</rdfs:label>
    <rdfs:comment>The amount of local SSD disks that will be attached to each preemptible worker node. Defaults to 0.</rdfs:comment>
    <rdfs:domain rdf:resource="http://example.org/onto/class/google_dataproc_cluster"/>
    <rdfs:range rdf:resource="http://www.w3.org/2001/XMLSchema#string"/>
  </owl:DatatypeProperty>
  <owl:DatatypeProperty rdf:about="http://example.org/onto/prop/google_dataproc_cluster_instance_selection_results">
    <rdfs:label>instance_selection_results</rdfs:label>
    <rdfs:comment>A list of instance selection results in the group.</rdfs:comment>
    <rdfs:domain rdf:resource="http://example.org/onto/class/google_dataproc_cluster"/>
    <rdfs:range rdf:resource="http://www.w3.org/2001/XMLSchema#string"/>
  </owl:DatatypeProperty>
  <owl:DatatypeProperty rdf:about="http://example.org/onto/prop/google_dataproc_cluster_machine_types">
    <rdfs:label>machine_types</rdfs:label>
    <rdfs:comment>Full machine-type names, e.g. "n1-standard-16".</rdfs:comment>
    <rdfs:domain rdf:resource="http://example.org/onto/class/google_dataproc_cluster"/>
    <rdfs:range rdf:resource="http://www.w3.org/2001/XMLSchema#string"/>
  </owl:DatatypeProperty>
  <owl:DatatypeProperty rdf:about="http://example.org/onto/prop/google_dataproc_cluster_rank">
    <rdfs:label>rank</rdfs:label>
    <rdfs:comment>Preference of this instance selection. Lower number means higher preference. Dataproc will first try to create a VM based on the machine-type with priority rank and fallback to next rank based on availability. Machine types and instance selections with the same priority have the same preference.</rdfs:comment>
    <rdfs:domain rdf:resource="http://example.org/onto/class/google_dataproc_cluster"/>
    <rdfs:range rdf:resource="http://www.w3.org/2001/XMLSchema#string"/>
  </owl:DatatypeProperty>
  <owl:DatatypeProperty rdf:about="http://example.org/onto/prop/google_dataproc_cluster_standard_capacity_base">
    <rdfs:label>standard_capacity_base</rdfs:label>
    <rdfs:comment>The base capacity that will always use Standard VMs to avoid risk of more preemption than the minimum capacity you need.</rdfs:comment>
    <rdfs:domain rdf:resource="http://example.org/onto/class/google_dataproc_cluster"/>
    <rdfs:range rdf:resource="http://www.w3.org/2001/XMLSchema#string"/>
  </owl:DatatypeProperty>
  <owl:DatatypeProperty rdf:about="http://example.org/onto/prop/google_dataproc_cluster_standard_capacity_percent_above_base">
    <rdfs:label>standard_capacity_percent_above_base</rdfs:label>
    <rdfs:comment>The percentage of target capacity that should use Standard VM. The remaining percentage will use Spot VMs.</rdfs:comment>
    <rdfs:domain rdf:resource="http://example.org/onto/class/google_dataproc_cluster"/>
    <rdfs:range rdf:resource="http://www.w3.org/2001/XMLSchema#string"/>
  </owl:DatatypeProperty>
  <owl:DatatypeProperty rdf:about="http://example.org/onto/prop/google_dataproc_cluster_user_service_account_mapping">
    <rdfs:label>user_service_account_mapping</rdfs:label>
    <rdfs:comment>User to service account mappings for multi-tenancy.</rdfs:comment>
    <rdfs:domain rdf:resource="http://example.org/onto/class/google_dataproc_cluster"/>
    <rdfs:range rdf:resource="http://www.w3.org/2001/XMLSchema#string"/>
  </owl:DatatypeProperty>
  <owl:DatatypeProperty rdf:about="http://example.org/onto/prop/google_dataproc_cluster_cross_realm_trust_admin_server">
    <rdfs:label>cross_realm_trust_admin_server</rdfs:label>
    <rdfs:comment>The admin server (IP or hostname) for the remote trusted realm in a cross realm trust relationship.</rdfs:comment>
    <rdfs:domain rdf:resource="http://example.org/onto/class/google_dataproc_cluster"/>
    <rdfs:range rdf:resource="http://www.w3.org/2001/XMLSchema#string"/>
  </owl:DatatypeProperty>
  <owl:DatatypeProperty rdf:about="http://example.org/onto/prop/google_dataproc_cluster_cross_realm_trust_kdc">
    <rdfs:label>cross_realm_trust_kdc</rdfs:label>
    <rdfs:comment>The KDC (IP or hostname) for the remote trusted realm in a cross realm trust relationship.</rdfs:comment>
    <rdfs:domain rdf:resource="http://example.org/onto/class/google_dataproc_cluster"/>
    <rdfs:range rdf:resource="http://www.w3.org/2001/XMLSchema#string"/>
  </owl:DatatypeProperty>
  <owl:DatatypeProperty rdf:about="http://example.org/onto/prop/google_dataproc_cluster_cross_realm_trust_realm">
    <rdfs:label>cross_realm_trust_realm</rdfs:label>
    <rdfs:comment>The remote realm the Dataproc on-cluster KDC will trust, should the user enable cross realm trust.</rdfs:comment>
    <rdfs:domain rdf:resource="http://example.org/onto/class/google_dataproc_cluster"/>
    <rdfs:range rdf:resource="http://www.w3.org/2001/XMLSchema#string"/>
  </owl:DatatypeProperty>
  <owl:DatatypeProperty rdf:about="http://example.org/onto/prop/google_dataproc_cluster_cross_realm_trust_shared_password_uri">
    <rdfs:label>cross_realm_trust_shared_password_uri</rdfs:label>
    <rdfs:comment>The Cloud Storage URI of a KMS encrypted file containing the shared password between the on-cluster
Kerberos realm and the remote trusted realm, in a cross realm trust relationship.</rdfs:comment>
    <rdfs:domain rdf:resource="http://example.org/onto/class/google_dataproc_cluster"/>
    <rdfs:range rdf:resource="http://www.w3.org/2001/XMLSchema#string"/>
  </owl:DatatypeProperty>
  <owl:DatatypeProperty rdf:about="http://example.org/onto/prop/google_dataproc_cluster_enable_kerberos">
    <rdfs:label>enable_kerberos</rdfs:label>
    <rdfs:comment>Flag to indicate whether to Kerberize the cluster.</rdfs:comment>
    <rdfs:domain rdf:resource="http://example.org/onto/class/google_dataproc_cluster"/>
    <rdfs:range rdf:resource="http://www.w3.org/2001/XMLSchema#string"/>
  </owl:DatatypeProperty>
  <owl:DatatypeProperty rdf:about="http://example.org/onto/prop/google_dataproc_cluster_kdc_db_key_uri">
    <rdfs:label>kdc_db_key_uri</rdfs:label>
    <rdfs:comment>The Cloud Storage URI of a KMS encrypted file containing the master key of the KDC database.</rdfs:comment>
    <rdfs:domain rdf:resource="http://example.org/onto/class/google_dataproc_cluster"/>
    <rdfs:range rdf:resource="http://www.w3.org/2001/XMLSchema#string"/>
  </owl:DatatypeProperty>
  <owl:DatatypeProperty rdf:about="http://example.org/onto/prop/google_dataproc_cluster_key_password_uri">
    <rdfs:label>key_password_uri</rdfs:label>
    <rdfs:comment>The Cloud Storage URI of a KMS encrypted file containing the password to the user provided key. For the self-signed certificate, this password is generated by Dataproc.</rdfs:comment>
    <rdfs:domain rdf:resource="http://example.org/onto/class/google_dataproc_cluster"/>
    <rdfs:range rdf:resource="http://www.w3.org/2001/XMLSchema#string"/>
  </owl:DatatypeProperty>
  <owl:DatatypeProperty rdf:about="http://example.org/onto/prop/google_dataproc_cluster_keystore_password_uri">
    <rdfs:label>keystore_password_uri</rdfs:label>
    <rdfs:comment>The Cloud Storage URI of a KMS encrypted file containing
the password to the user provided keystore. For the self-signed certificate, this password is generated
by Dataproc</rdfs:comment>
    <rdfs:domain rdf:resource="http://example.org/onto/class/google_dataproc_cluster"/>
    <rdfs:range rdf:resource="http://www.w3.org/2001/XMLSchema#string"/>
  </owl:DatatypeProperty>
  <owl:DatatypeProperty rdf:about="http://example.org/onto/prop/google_dataproc_cluster_keystore_uri">
    <rdfs:label>keystore_uri</rdfs:label>
    <rdfs:comment>The Cloud Storage URI of the keystore file used for SSL encryption. If not provided, Dataproc will provide a self-signed certificate.</rdfs:comment>
    <rdfs:domain rdf:resource="http://example.org/onto/class/google_dataproc_cluster"/>
    <rdfs:range rdf:resource="http://www.w3.org/2001/XMLSchema#string"/>
  </owl:DatatypeProperty>
  <owl:DatatypeProperty rdf:about="http://example.org/onto/prop/google_dataproc_cluster_kms_key_uri">
    <rdfs:label>kms_key_uri</rdfs:label>
    <rdfs:comment>The uri of the KMS key used to encrypt various sensitive files.</rdfs:comment>
    <rdfs:domain rdf:resource="http://example.org/onto/class/google_dataproc_cluster"/>
    <rdfs:range rdf:resource="http://www.w3.org/2001/XMLSchema#string"/>
  </owl:DatatypeProperty>
  <owl:DatatypeProperty rdf:about="http://example.org/onto/prop/google_dataproc_cluster_realm">
    <rdfs:label>realm</rdfs:label>
    <rdfs:comment>The name of the on-cluster Kerberos realm. If not specified, the uppercased domain of hostnames will be the realm.</rdfs:comment>
    <rdfs:domain rdf:resource="http://example.org/onto/class/google_dataproc_cluster"/>
    <rdfs:range rdf:resource="http://www.w3.org/2001/XMLSchema#string"/>
  </owl:DatatypeProperty>
  <owl:DatatypeProperty rdf:about="http://example.org/onto/prop/google_dataproc_cluster_root_principal_password_uri">
    <rdfs:label>root_principal_password_uri</rdfs:label>
    <rdfs:comment>The cloud Storage URI of a KMS encrypted file containing the root principal password.</rdfs:comment>
    <rdfs:domain rdf:resource="http://example.org/onto/class/google_dataproc_cluster"/>
    <rdfs:range rdf:resource="http://www.w3.org/2001/XMLSchema#string"/>
  </owl:DatatypeProperty>
  <owl:DatatypeProperty rdf:about="http://example.org/onto/prop/google_dataproc_cluster_tgt_lifetime_hours">
    <rdfs:label>tgt_lifetime_hours</rdfs:label>
    <rdfs:comment>The lifetime of the ticket granting ticket, in hours.</rdfs:comment>
    <rdfs:domain rdf:resource="http://example.org/onto/class/google_dataproc_cluster"/>
    <rdfs:range rdf:resource="http://www.w3.org/2001/XMLSchema#string"/>
  </owl:DatatypeProperty>
  <owl:DatatypeProperty rdf:about="http://example.org/onto/prop/google_dataproc_cluster_truststore_password_uri">
    <rdfs:label>truststore_password_uri</rdfs:label>
    <rdfs:comment>The Cloud Storage URI of a KMS encrypted file containing the password to the user provided truststore. For the self-signed certificate, this password is generated by Dataproc.</rdfs:comment>
    <rdfs:domain rdf:resource="http://example.org/onto/class/google_dataproc_cluster"/>
    <rdfs:range rdf:resource="http://www.w3.org/2001/XMLSchema#string"/>
  </owl:DatatypeProperty>
  <owl:DatatypeProperty rdf:about="http://example.org/onto/prop/google_dataproc_cluster_truststore_uri">
    <rdfs:label>truststore_uri</rdfs:label>
    <rdfs:comment>The Cloud Storage URI of the truststore file used for SSL encryption. If not provided, Dataproc will provide a self-signed certificate.</rdfs:comment>
    <rdfs:domain rdf:resource="http://example.org/onto/class/google_dataproc_cluster"/>
    <rdfs:range rdf:resource="http://www.w3.org/2001/XMLSchema#string"/>
  </owl:DatatypeProperty>
  <owl:DatatypeProperty rdf:about="http://example.org/onto/prop/google_dataproc_cluster_image_version">
    <rdfs:label>image_version</rdfs:label>
    <rdfs:comment>The Cloud Dataproc image version to use for the cluster - this controls the sets of software versions installed onto the nodes when you create clusters. If not specified, defaults to the latest version.</rdfs:comment>
    <rdfs:domain rdf:resource="http://example.org/onto/class/google_dataproc_cluster"/>
    <rdfs:range rdf:resource="http://www.w3.org/2001/XMLSchema#string"/>
  </owl:DatatypeProperty>
  <owl:DatatypeProperty rdf:about="http://example.org/onto/prop/google_dataproc_cluster_optional_components">
    <rdfs:label>optional_components</rdfs:label>
    <rdfs:comment>The set of optional components to activate on the cluster.</rdfs:comment>
    <rdfs:domain rdf:resource="http://example.org/onto/class/google_dataproc_cluster"/>
    <rdfs:range rdf:resource="http://www.w3.org/2001/XMLSchema#string"/>
  </owl:DatatypeProperty>
  <owl:DatatypeProperty rdf:about="http://example.org/onto/prop/google_dataproc_cluster_override_properties">
    <rdfs:label>override_properties</rdfs:label>
    <rdfs:comment>A list of override and additional properties (key/value pairs) used to modify various aspects of the common configuration files used when creating a cluster.</rdfs:comment>
    <rdfs:domain rdf:resource="http://example.org/onto/class/google_dataproc_cluster"/>
    <rdfs:range rdf:resource="http://www.w3.org/2001/XMLSchema#string"/>
  </owl:DatatypeProperty>
  <owl:DatatypeProperty rdf:about="http://example.org/onto/prop/google_dataproc_cluster_properties">
    <rdfs:label>properties</rdfs:label>
    <rdfs:comment>A list of the properties used to set the daemon config files. This will include any values supplied by the user via cluster_config.software_config.override_properties</rdfs:comment>
    <rdfs:domain rdf:resource="http://example.org/onto/class/google_dataproc_cluster"/>
    <rdfs:range rdf:resource="http://www.w3.org/2001/XMLSchema#string"/>
  </owl:DatatypeProperty>
  <owl:DatatypeProperty rdf:about="http://example.org/onto/prop/google_dataproc_cluster_image_uri">
    <rdfs:label>image_uri</rdfs:label>
    <rdfs:comment>The URI for the image to use for this master/worker</rdfs:comment>
    <rdfs:domain rdf:resource="http://example.org/onto/class/google_dataproc_cluster"/>
    <rdfs:range rdf:resource="http://www.w3.org/2001/XMLSchema#string"/>
  </owl:DatatypeProperty>
  <owl:DatatypeProperty rdf:about="http://example.org/onto/prop/google_dataproc_cluster_instance_names">
    <rdfs:label>instance_names</rdfs:label>
    <rdfs:comment>List of master/worker instance names which have been assigned to the cluster.</rdfs:comment>
    <rdfs:domain rdf:resource="http://example.org/onto/class/google_dataproc_cluster"/>
    <rdfs:range rdf:resource="http://www.w3.org/2001/XMLSchema#string"/>
  </owl:DatatypeProperty>
  <owl:DatatypeProperty rdf:about="http://example.org/onto/prop/google_dataproc_cluster_machine_type">
    <rdfs:label>machine_type</rdfs:label>
    <rdfs:comment>The name of a Google Compute Engine machine type to create for the master/worker</rdfs:comment>
    <rdfs:domain rdf:resource="http://example.org/onto/class/google_dataproc_cluster"/>
    <rdfs:range rdf:resource="http://www.w3.org/2001/XMLSchema#string"/>
  </owl:DatatypeProperty>
  <owl:DatatypeProperty rdf:about="http://example.org/onto/prop/google_dataproc_cluster_min_cpu_platform">
    <rdfs:label>min_cpu_platform</rdfs:label>
    <rdfs:comment>The name of a minimum generation of CPU family for the master/worker. If not specified, GCP will default to a predetermined computed value for each zone.</rdfs:comment>
    <rdfs:domain rdf:resource="http://example.org/onto/class/google_dataproc_cluster"/>
    <rdfs:range rdf:resource="http://www.w3.org/2001/XMLSchema#string"/>
  </owl:DatatypeProperty>
  <owl:DatatypeProperty rdf:about="http://example.org/onto/prop/google_dataproc_cluster_min_num_instances">
    <rdfs:label>min_num_instances</rdfs:label>
    <rdfs:comment>The minimum number of primary worker instances to create.</rdfs:comment>
    <rdfs:domain rdf:resource="http://example.org/onto/class/google_dataproc_cluster"/>
    <rdfs:range rdf:resource="http://www.w3.org/2001/XMLSchema#string"/>
  </owl:DatatypeProperty>
  <owl:DatatypeProperty rdf:about="http://example.org/onto/prop/google_dataproc_cluster_num_instances">
    <rdfs:label>num_instances</rdfs:label>
    <rdfs:comment>Specifies the number of worker nodes to create. If not specified, GCP will default to a predetermined computed value.</rdfs:comment>
    <rdfs:domain rdf:resource="http://example.org/onto/class/google_dataproc_cluster"/>
    <rdfs:range rdf:resource="http://www.w3.org/2001/XMLSchema#string"/>
  </owl:DatatypeProperty>
  <owl:DatatypeProperty rdf:about="http://example.org/onto/prop/google_dataproc_cluster_accelerator_count">
    <rdfs:label>accelerator_count</rdfs:label>
    <rdfs:comment>The number of the accelerator cards of this type exposed to this instance. Often restricted to one of 1, 2, 4, or 8.</rdfs:comment>
    <rdfs:domain rdf:resource="http://example.org/onto/class/google_dataproc_cluster"/>
    <rdfs:range rdf:resource="http://www.w3.org/2001/XMLSchema#string"/>
  </owl:DatatypeProperty>
  <owl:DatatypeProperty rdf:about="http://example.org/onto/prop/google_dataproc_cluster_accelerator_type">
    <rdfs:label>accelerator_type</rdfs:label>
    <rdfs:comment>The short name of the accelerator type to expose to this instance. For example, nvidia-tesla-k80.</rdfs:comment>
    <rdfs:domain rdf:resource="http://example.org/onto/class/google_dataproc_cluster"/>
    <rdfs:range rdf:resource="http://www.w3.org/2001/XMLSchema#string"/>
  </owl:DatatypeProperty>
  <owl:DatatypeProperty rdf:about="http://example.org/onto/prop/google_dataproc_cluster_boot_disk_size_gb">
    <rdfs:label>boot_disk_size_gb</rdfs:label>
    <rdfs:comment>Size of the primary disk attached to each node, specified in GB. The primary disk contains the boot volume and system libraries, and the smallest allowed disk size is 10GB. GCP will default to a predetermined computed value if not set (currently 500GB). Note: If SSDs are not attached, it also contains the HDFS data blocks and Hadoop working directories.</rdfs:comment>
    <rdfs:domain rdf:resource="http://example.org/onto/class/google_dataproc_cluster"/>
    <rdfs:range rdf:resource="http://www.w3.org/2001/XMLSchema#string"/>
  </owl:DatatypeProperty>
  <owl:DatatypeProperty rdf:about="http://example.org/onto/prop/google_dataproc_cluster_boot_disk_type">
    <rdfs:label>boot_disk_type</rdfs:label>
    <rdfs:comment>The disk type of the primary disk attached to each node. Such as "pd-ssd" or "pd-standard". Defaults to "pd-standard".</rdfs:comment>
    <rdfs:domain rdf:resource="http://example.org/onto/class/google_dataproc_cluster"/>
    <rdfs:range rdf:resource="http://www.w3.org/2001/XMLSchema#string"/>
  </owl:DatatypeProperty>
  <owl:DatatypeProperty rdf:about="http://example.org/onto/prop/google_dataproc_cluster_local_ssd_interface">
    <rdfs:label>local_ssd_interface</rdfs:label>
    <rdfs:comment>Interface type of local SSDs (default is "scsi"). Valid values: "scsi" (Small Computer System Interface), "nvme" (Non-Volatile Memory Express).</rdfs:comment>
    <rdfs:domain rdf:resource="http://example.org/onto/class/google_dataproc_cluster"/>
    <rdfs:range rdf:resource="http://www.w3.org/2001/XMLSchema#string"/>
  </owl:DatatypeProperty>
  <owl:DatatypeProperty rdf:about="http://example.org/onto/prop/google_dataproc_cluster_num_local_ssds">
    <rdfs:label>num_local_ssds</rdfs:label>
    <rdfs:comment>The amount of local SSD disks that will be attached to each master cluster node. Defaults to 0.</rdfs:comment>
    <rdfs:domain rdf:resource="http://example.org/onto/class/google_dataproc_cluster"/>
    <rdfs:range rdf:resource="http://www.w3.org/2001/XMLSchema#string"/>
  </owl:DatatypeProperty>
  <owl:DatatypeProperty rdf:about="http://example.org/onto/prop/google_dataproc_cluster_create">
    <rdfs:label>create</rdfs:label>
    <rdfs:domain rdf:resource="http://example.org/onto/class/google_dataproc_cluster"/>
    <rdfs:range rdf:resource="http://www.w3.org/2001/XMLSchema#string"/>
  </owl:DatatypeProperty>
  <owl:DatatypeProperty rdf:about="http://example.org/onto/prop/google_dataproc_cluster_delete">
    <rdfs:label>delete</rdfs:label>
    <rdfs:domain rdf:resource="http://example.org/onto/class/google_dataproc_cluster"/>
    <rdfs:range rdf:resource="http://www.w3.org/2001/XMLSchema#string"/>
  </owl:DatatypeProperty>
  <owl:DatatypeProperty rdf:about="http://example.org/onto/prop/google_dataproc_cluster_update">
    <rdfs:label>update</rdfs:label>
    <rdfs:domain rdf:resource="http://example.org/onto/class/google_dataproc_cluster"/>
    <rdfs:range rdf:resource="http://www.w3.org/2001/XMLSchema#string"/>
  </owl:DatatypeProperty>
  <owl:DatatypeProperty rdf:about="http://example.org/onto/prop/google_dataproc_cluster_staging_bucket">
    <rdfs:label>staging_bucket</rdfs:label>
    <rdfs:comment>A Cloud Storage bucket used to stage job dependencies, config files, and job driver console output. If you do not specify a staging bucket, Cloud Dataproc will determine a Cloud Storage location (US, ASIA, or EU) for your cluster's staging bucket according to the Compute Engine zone where your cluster is deployed, and then create and manage this project-level, per-location bucket.</rdfs:comment>
    <rdfs:domain rdf:resource="http://example.org/onto/class/google_dataproc_cluster"/>
    <rdfs:range rdf:resource="http://www.w3.org/2001/XMLSchema#string"/>
  </owl:DatatypeProperty>
  <owl:DatatypeProperty rdf:about="http://example.org/onto/prop/google_dataproc_cluster_dataproc_metastore_service">
    <rdfs:label>dataproc_metastore_service</rdfs:label>
    <rdfs:comment>The Hive Metastore configuration for this workload.</rdfs:comment>
    <rdfs:domain rdf:resource="http://example.org/onto/class/google_dataproc_cluster"/>
    <rdfs:range rdf:resource="http://www.w3.org/2001/XMLSchema#string"/>
  </owl:DatatypeProperty>
  <owl:DatatypeProperty rdf:about="http://example.org/onto/prop/google_dataproc_cluster_dataproc_cluster">
    <rdfs:label>dataproc_cluster</rdfs:label>
    <rdfs:comment>Resource name of an existing Dataproc Cluster to act as a Spark History Server for the workload.</rdfs:comment>
    <rdfs:domain rdf:resource="http://example.org/onto/class/google_dataproc_cluster"/>
    <rdfs:range rdf:resource="http://www.w3.org/2001/XMLSchema#string"/>
  </owl:DatatypeProperty>
  <owl:DatatypeProperty rdf:about="http://example.org/onto/prop/google_dataproc_cluster_kubernetes_namespace">
    <rdfs:label>kubernetes_namespace</rdfs:label>
    <rdfs:comment>A namespace within the Kubernetes cluster to deploy into. If this namespace does not exist, it is created. If it exists, Dataproc verifies that another Dataproc VirtualCluster is not installed into it. If not specified, the name of the Dataproc Cluster is used.</rdfs:comment>
    <rdfs:domain rdf:resource="http://example.org/onto/class/google_dataproc_cluster"/>
    <rdfs:range rdf:resource="http://www.w3.org/2001/XMLSchema#string"/>
  </owl:DatatypeProperty>
  <owl:DatatypeProperty rdf:about="http://example.org/onto/prop/google_dataproc_cluster_gke_cluster_target">
    <rdfs:label>gke_cluster_target</rdfs:label>
    <rdfs:comment>A target GKE cluster to deploy to. It must be in the same project and region as the Dataproc cluster (the GKE cluster can be zonal or regional). Format: 'projects/{project}/locations/{location}/clusters/{cluster_id}'</rdfs:comment>
    <rdfs:domain rdf:resource="http://example.org/onto/class/google_dataproc_cluster"/>
    <rdfs:range rdf:resource="http://www.w3.org/2001/XMLSchema#string"/>
  </owl:DatatypeProperty>
  <owl:DatatypeProperty rdf:about="http://example.org/onto/prop/google_dataproc_cluster_node_pool">
    <rdfs:label>node_pool</rdfs:label>
    <rdfs:comment>The target GKE node pool. Format: 'projects/{project}/locations/{location}/clusters/{cluster}/nodePools/{nodePool}'</rdfs:comment>
    <rdfs:domain rdf:resource="http://example.org/onto/class/google_dataproc_cluster"/>
    <rdfs:range rdf:resource="http://www.w3.org/2001/XMLSchema#string"/>
  </owl:DatatypeProperty>
  <owl:DatatypeProperty rdf:about="http://example.org/onto/prop/google_dataproc_cluster_roles">
    <rdfs:label>roles</rdfs:label>
    <rdfs:comment>The roles associated with the GKE node pool.</rdfs:comment>
    <rdfs:domain rdf:resource="http://example.org/onto/class/google_dataproc_cluster"/>
    <rdfs:range rdf:resource="http://www.w3.org/2001/XMLSchema#string"/>
  </owl:DatatypeProperty>
  <owl:DatatypeProperty rdf:about="http://example.org/onto/prop/google_dataproc_cluster_locations">
    <rdfs:label>locations</rdfs:label>
    <rdfs:comment>The list of Compute Engine zones where node pool nodes associated with a Dataproc on GKE virtual cluster will be located.</rdfs:comment>
    <rdfs:domain rdf:resource="http://example.org/onto/class/google_dataproc_cluster"/>
    <rdfs:range rdf:resource="http://www.w3.org/2001/XMLSchema#string"/>
  </owl:DatatypeProperty>
  <owl:DatatypeProperty rdf:about="http://example.org/onto/prop/google_dataproc_cluster_max_node_count">
    <rdfs:label>max_node_count</rdfs:label>
    <rdfs:comment>The maximum number of nodes in the node pool. Must be >= minNodeCount, and must be > 0.</rdfs:comment>
    <rdfs:domain rdf:resource="http://example.org/onto/class/google_dataproc_cluster"/>
    <rdfs:range rdf:resource="http://www.w3.org/2001/XMLSchema#string"/>
  </owl:DatatypeProperty>
  <owl:DatatypeProperty rdf:about="http://example.org/onto/prop/google_dataproc_cluster_min_node_count">
    <rdfs:label>min_node_count</rdfs:label>
    <rdfs:comment>The minimum number of nodes in the node pool. Must be >= 0 and <= maxNodeCount.</rdfs:comment>
    <rdfs:domain rdf:resource="http://example.org/onto/class/google_dataproc_cluster"/>
    <rdfs:range rdf:resource="http://www.w3.org/2001/XMLSchema#string"/>
  </owl:DatatypeProperty>
  <owl:DatatypeProperty rdf:about="http://example.org/onto/prop/google_dataproc_cluster_local_ssd_count">
    <rdfs:label>local_ssd_count</rdfs:label>
    <rdfs:comment>The minimum number of nodes in the node pool. Must be >= 0 and <= maxNodeCount.</rdfs:comment>
    <rdfs:domain rdf:resource="http://example.org/onto/class/google_dataproc_cluster"/>
    <rdfs:range rdf:resource="http://www.w3.org/2001/XMLSchema#string"/>
  </owl:DatatypeProperty>
  <owl:DatatypeProperty rdf:about="http://example.org/onto/prop/google_dataproc_cluster_machine_type">
    <rdfs:label>machine_type</rdfs:label>
    <rdfs:comment>The name of a Compute Engine machine type.</rdfs:comment>
    <rdfs:domain rdf:resource="http://example.org/onto/class/google_dataproc_cluster"/>
    <rdfs:range rdf:resource="http://www.w3.org/2001/XMLSchema#string"/>
  </owl:DatatypeProperty>
  <owl:DatatypeProperty rdf:about="http://example.org/onto/prop/google_dataproc_cluster_min_cpu_platform">
    <rdfs:label>min_cpu_platform</rdfs:label>
    <rdfs:comment>Minimum CPU platform to be used by this instance. The instance may be scheduled on the specified or a newer CPU platform. Specify the friendly names of CPU platforms, such as "Intel Haswell" or "Intel Sandy Bridge".</rdfs:comment>
    <rdfs:domain rdf:resource="http://example.org/onto/class/google_dataproc_cluster"/>
    <rdfs:range rdf:resource="http://www.w3.org/2001/XMLSchema#string"/>
  </owl:DatatypeProperty>
  <owl:DatatypeProperty rdf:about="http://example.org/onto/prop/google_dataproc_cluster_preemptible">
    <rdfs:label>preemptible</rdfs:label>
    <rdfs:comment>Whether the nodes are created as preemptible VM instances. Preemptible nodes cannot be used in a node pool with the CONTROLLER role or in the DEFAULT node pool if the CONTROLLER role is not assigned (the DEFAULT node pool will assume the CONTROLLER role).</rdfs:comment>
    <rdfs:domain rdf:resource="http://example.org/onto/class/google_dataproc_cluster"/>
    <rdfs:range rdf:resource="http://www.w3.org/2001/XMLSchema#string"/>
  </owl:DatatypeProperty>
  <owl:DatatypeProperty rdf:about="http://example.org/onto/prop/google_dataproc_cluster_spot">
    <rdfs:label>spot</rdfs:label>
    <rdfs:comment>Spot flag for enabling Spot VM, which is a rebrand of the existing preemptible flag.</rdfs:comment>
    <rdfs:domain rdf:resource="http://example.org/onto/class/google_dataproc_cluster"/>
    <rdfs:range rdf:resource="http://www.w3.org/2001/XMLSchema#string"/>
  </owl:DatatypeProperty>
  <owl:DatatypeProperty rdf:about="http://example.org/onto/prop/google_dataproc_cluster_component_version">
    <rdfs:label>component_version</rdfs:label>
    <rdfs:comment>The components that should be installed in this Dataproc cluster. The key must be a string from the KubernetesComponent enumeration. The value is the version of the software to be installed.</rdfs:comment>
    <rdfs:domain rdf:resource="http://example.org/onto/class/google_dataproc_cluster"/>
    <rdfs:range rdf:resource="http://www.w3.org/2001/XMLSchema#string"/>
  </owl:DatatypeProperty>
  <owl:DatatypeProperty rdf:about="http://example.org/onto/prop/google_dataproc_cluster_properties">
    <rdfs:label>properties</rdfs:label>
    <rdfs:comment>The properties to set on daemon config files. Property keys are specified in prefix:property format, for example spark:spark.kubernetes.container.image.</rdfs:comment>
    <rdfs:domain rdf:resource="http://example.org/onto/class/google_dataproc_cluster"/>
    <rdfs:range rdf:resource="http://www.w3.org/2001/XMLSchema#string"/>
  </owl:DatatypeProperty>
</rdf:RDF>
