<?xml version="1.0" encoding="UTF-8"?>
<rdf:RDF
  xmlns:rdf="http://www.w3.org/1999/02/22-rdf-syntax-ns#"
  xmlns:rdfs="http://www.w3.org/2000/01/rdf-schema#"
  xmlns:owl="http://www.w3.org/2002/07/owl#"
  xmlns:xsd="http://www.w3.org/2001/XMLSchema#"
  xml:base="http://example.org/onto/">
  <owl:Class rdf:about="http://example.org/onto/class/google_compute_storage_pool">
    <rdfs:label>google_compute_storage_pool</rdfs:label>
    <rdfs:comment>#
#     ***     AUTO GENERATED CODE    ***    Type: MMv1     ***
#
# ----------------------------------------------------------------------------
#
#     This code is generated by Magic Modules using the following:
#
#     Configuration: https:#github.com/GoogleCloudPlatform/magic-modules/tree/main/mmv1/products/compute/StoragePool.yaml
#     Template:      https:#github.com/GoogleCloudPlatform/magic-modules/tree/main/mmv1/templates/terraform/resource.html.markdown.tmpl
#
#     DO NOT EDIT this file directly. Any changes made to this file will be
#     overwritten during the next generation cycle.
#
# ----------------------------------------------------------------------------
subcategory: "Compute Engine"
description: |-
  A Hyperdisk Storage Pool is a pre-purchased collection of capacity, throughput, and IOPS
  which you can then provision to your applications as needed.
---</rdfs:comment>
  </owl:Class>
  <owl:DatatypeProperty rdf:about="http://example.org/onto/prop/google_compute_storage_pool_capacity_provisioning_type">
    <rdfs:label>capacity_provisioning_type</rdfs:label>
    <rdfs:comment>Provisioning type of the byte capacity of the pool. Possible values: ["STANDARD", "ADVANCED"]</rdfs:comment>
    <rdfs:domain rdf:resource="http://example.org/onto/class/google_compute_storage_pool"/>
    <rdfs:range rdf:resource="http://www.w3.org/2001/XMLSchema#string"/>
  </owl:DatatypeProperty>
  <owl:DatatypeProperty rdf:about="http://example.org/onto/prop/google_compute_storage_pool_creation_timestamp">
    <rdfs:label>creation_timestamp</rdfs:label>
    <rdfs:comment>Creation timestamp in RFC3339 text format.</rdfs:comment>
    <rdfs:domain rdf:resource="http://example.org/onto/class/google_compute_storage_pool"/>
    <rdfs:range rdf:resource="http://www.w3.org/2001/XMLSchema#string"/>
  </owl:DatatypeProperty>
  <owl:DatatypeProperty rdf:about="http://example.org/onto/prop/google_compute_storage_pool_deletion_protection">
    <rdfs:label>deletion_protection</rdfs:label>
    <rdfs:comment>Whether Terraform will be prevented from destroying the StoragePool.
When the field is set to true or unset in Terraform state, a 'terraform apply'
or 'terraform destroy' that would delete the StoragePool will fail.
When the field is set to false, deleting the StoragePool is allowed.</rdfs:comment>
    <rdfs:domain rdf:resource="http://example.org/onto/class/google_compute_storage_pool"/>
    <rdfs:range rdf:resource="http://www.w3.org/2001/XMLSchema#string"/>
  </owl:DatatypeProperty>
  <owl:DatatypeProperty rdf:about="http://example.org/onto/prop/google_compute_storage_pool_description">
    <rdfs:label>description</rdfs:label>
    <rdfs:comment>A description of this resource. Provide this property when you create the resource.</rdfs:comment>
    <rdfs:domain rdf:resource="http://example.org/onto/class/google_compute_storage_pool"/>
    <rdfs:range rdf:resource="http://www.w3.org/2001/XMLSchema#string"/>
  </owl:DatatypeProperty>
  <owl:DatatypeProperty rdf:about="http://example.org/onto/prop/google_compute_storage_pool_effective_labels">
    <rdfs:label>effective_labels</rdfs:label>
    <rdfs:comment>All of labels (key/value pairs) present on the resource in GCP, including the labels configured through Terraform, other clients and services.</rdfs:comment>
    <rdfs:domain rdf:resource="http://example.org/onto/class/google_compute_storage_pool"/>
    <rdfs:range rdf:resource="http://www.w3.org/2001/XMLSchema#string"/>
  </owl:DatatypeProperty>
  <owl:DatatypeProperty rdf:about="http://example.org/onto/prop/google_compute_storage_pool_id">
    <rdfs:label>id</rdfs:label>
    <rdfs:comment>The unique identifier for the resource. This identifier is defined by the server.</rdfs:comment>
    <rdfs:domain rdf:resource="http://example.org/onto/class/google_compute_storage_pool"/>
    <rdfs:range rdf:resource="http://www.w3.org/2001/XMLSchema#string"/>
  </owl:DatatypeProperty>
  <owl:DatatypeProperty rdf:about="http://example.org/onto/prop/google_compute_storage_pool_kind">
    <rdfs:label>kind</rdfs:label>
    <rdfs:comment>Type of the resource.</rdfs:comment>
    <rdfs:domain rdf:resource="http://example.org/onto/class/google_compute_storage_pool"/>
    <rdfs:range rdf:resource="http://www.w3.org/2001/XMLSchema#string"/>
  </owl:DatatypeProperty>
  <owl:DatatypeProperty rdf:about="http://example.org/onto/prop/google_compute_storage_pool_label_fingerprint">
    <rdfs:label>label_fingerprint</rdfs:label>
    <rdfs:comment>The fingerprint used for optimistic locking of this resource.
Used internally during updates.</rdfs:comment>
    <rdfs:domain rdf:resource="http://example.org/onto/class/google_compute_storage_pool"/>
    <rdfs:range rdf:resource="http://www.w3.org/2001/XMLSchema#string"/>
  </owl:DatatypeProperty>
  <owl:DatatypeProperty rdf:about="http://example.org/onto/prop/google_compute_storage_pool_labels">
    <rdfs:label>labels</rdfs:label>
    <rdfs:comment>Labels to apply to this storage pool. These can be later modified by the setLabels method.


**Note**: This field is non-authoritative, and will only manage the labels present in your configuration.
Please refer to the field 'effective_labels' for all of the labels present on the resource.</rdfs:comment>
    <rdfs:domain rdf:resource="http://example.org/onto/class/google_compute_storage_pool"/>
    <rdfs:range rdf:resource="http://www.w3.org/2001/XMLSchema#string"/>
  </owl:DatatypeProperty>
  <owl:DatatypeProperty rdf:about="http://example.org/onto/prop/google_compute_storage_pool_name">
    <rdfs:label>name</rdfs:label>
    <rdfs:comment>Name of the resource. Provided by the client when the resource is created.
The name must be 1-63 characters long, and comply with RFC1035.
Specifically, the name must be 1-63 characters long and match
the regular expression '[a-z]([-a-z0-9]*[a-z0-9])?'
which means the first character must be a lowercase letter,
and all following characters must be a dash, lowercase letter, or digit,
except the last character, which cannot be a dash.</rdfs:comment>
    <rdfs:domain rdf:resource="http://example.org/onto/class/google_compute_storage_pool"/>
    <rdfs:range rdf:resource="http://www.w3.org/2001/XMLSchema#string"/>
  </owl:DatatypeProperty>
  <owl:DatatypeProperty rdf:about="http://example.org/onto/prop/google_compute_storage_pool_performance_provisioning_type">
    <rdfs:label>performance_provisioning_type</rdfs:label>
    <rdfs:comment>Provisioning type of the performance-related parameters of the pool, such as throughput and IOPS. Possible values: ["STANDARD", "ADVANCED"]</rdfs:comment>
    <rdfs:domain rdf:resource="http://example.org/onto/class/google_compute_storage_pool"/>
    <rdfs:range rdf:resource="http://www.w3.org/2001/XMLSchema#string"/>
  </owl:DatatypeProperty>
  <owl:DatatypeProperty rdf:about="http://example.org/onto/prop/google_compute_storage_pool_pool_provisioned_capacity_gb">
    <rdfs:label>pool_provisioned_capacity_gb</rdfs:label>
    <rdfs:comment>Size, in GiB, of the storage pool. For more information about the size limits,
see https://cloud.google.com/compute/docs/disks/storage-pools.</rdfs:comment>
    <rdfs:domain rdf:resource="http://example.org/onto/class/google_compute_storage_pool"/>
    <rdfs:range rdf:resource="http://www.w3.org/2001/XMLSchema#string"/>
  </owl:DatatypeProperty>
  <owl:DatatypeProperty rdf:about="http://example.org/onto/prop/google_compute_storage_pool_pool_provisioned_iops">
    <rdfs:label>pool_provisioned_iops</rdfs:label>
    <rdfs:comment>Provisioned IOPS of the storage pool.
Only relevant if the storage pool type is 'hyperdisk-balanced'.</rdfs:comment>
    <rdfs:domain rdf:resource="http://example.org/onto/class/google_compute_storage_pool"/>
    <rdfs:range rdf:resource="http://www.w3.org/2001/XMLSchema#string"/>
  </owl:DatatypeProperty>
  <owl:DatatypeProperty rdf:about="http://example.org/onto/prop/google_compute_storage_pool_pool_provisioned_throughput">
    <rdfs:label>pool_provisioned_throughput</rdfs:label>
    <rdfs:comment>Provisioned throughput, in MB/s, of the storage pool.
Only relevant if the storage pool type is 'hyperdisk-balanced' or 'hyperdisk-throughput'.</rdfs:comment>
    <rdfs:domain rdf:resource="http://example.org/onto/class/google_compute_storage_pool"/>
    <rdfs:range rdf:resource="http://www.w3.org/2001/XMLSchema#string"/>
  </owl:DatatypeProperty>
  <owl:DatatypeProperty rdf:about="http://example.org/onto/prop/google_compute_storage_pool_project">
    <rdfs:label>project</rdfs:label>
    <rdfs:domain rdf:resource="http://example.org/onto/class/google_compute_storage_pool"/>
    <rdfs:range rdf:resource="http://www.w3.org/2001/XMLSchema#string"/>
  </owl:DatatypeProperty>
  <owl:DatatypeProperty rdf:about="http://example.org/onto/prop/google_compute_storage_pool_resource_status">
    <rdfs:label>resource_status</rdfs:label>
    <rdfs:comment>Status information for the storage pool resource.</rdfs:comment>
    <rdfs:domain rdf:resource="http://example.org/onto/class/google_compute_storage_pool"/>
    <rdfs:range rdf:resource="http://www.w3.org/2001/XMLSchema#string"/>
  </owl:DatatypeProperty>
  <owl:DatatypeProperty rdf:about="http://example.org/onto/prop/google_compute_storage_pool_status">
    <rdfs:label>status</rdfs:label>
    <rdfs:comment>Status information for the storage pool resource.</rdfs:comment>
    <rdfs:domain rdf:resource="http://example.org/onto/class/google_compute_storage_pool"/>
    <rdfs:range rdf:resource="http://www.w3.org/2001/XMLSchema#string"/>
  </owl:DatatypeProperty>
  <owl:DatatypeProperty rdf:about="http://example.org/onto/prop/google_compute_storage_pool_storage_pool_type">
    <rdfs:label>storage_pool_type</rdfs:label>
    <rdfs:comment>Type of the storage pool. For example, the
following are valid values:

* 'https://www.googleapis.com/compute/v1/projects/{project_id}/zones/{zone}/storagePoolTypes/hyperdisk-balanced'
* 'hyperdisk-throughput'</rdfs:comment>
    <rdfs:domain rdf:resource="http://example.org/onto/class/google_compute_storage_pool"/>
    <rdfs:range rdf:resource="http://www.w3.org/2001/XMLSchema#string"/>
  </owl:DatatypeProperty>
  <owl:DatatypeProperty rdf:about="http://example.org/onto/prop/google_compute_storage_pool_terraform_labels">
    <rdfs:label>terraform_labels</rdfs:label>
    <rdfs:comment>The combination of labels configured directly on the resource
 and default labels configured on the provider.</rdfs:comment>
    <rdfs:domain rdf:resource="http://example.org/onto/class/google_compute_storage_pool"/>
    <rdfs:range rdf:resource="http://www.w3.org/2001/XMLSchema#string"/>
  </owl:DatatypeProperty>
  <owl:DatatypeProperty rdf:about="http://example.org/onto/prop/google_compute_storage_pool_zone">
    <rdfs:label>zone</rdfs:label>
    <rdfs:comment>A reference to the zone where the storage pool resides.</rdfs:comment>
    <rdfs:domain rdf:resource="http://example.org/onto/class/google_compute_storage_pool"/>
    <rdfs:range rdf:resource="http://www.w3.org/2001/XMLSchema#string"/>
  </owl:DatatypeProperty>
  <owl:DatatypeProperty rdf:about="http://example.org/onto/prop/google_compute_storage_pool_create">
    <rdfs:label>create</rdfs:label>
    <rdfs:domain rdf:resource="http://example.org/onto/class/google_compute_storage_pool"/>
    <rdfs:range rdf:resource="http://www.w3.org/2001/XMLSchema#string"/>
  </owl:DatatypeProperty>
  <owl:DatatypeProperty rdf:about="http://example.org/onto/prop/google_compute_storage_pool_delete">
    <rdfs:label>delete</rdfs:label>
    <rdfs:domain rdf:resource="http://example.org/onto/class/google_compute_storage_pool"/>
    <rdfs:range rdf:resource="http://www.w3.org/2001/XMLSchema#string"/>
  </owl:DatatypeProperty>
  <owl:DatatypeProperty rdf:about="http://example.org/onto/prop/google_compute_storage_pool_update">
    <rdfs:label>update</rdfs:label>
    <rdfs:domain rdf:resource="http://example.org/onto/class/google_compute_storage_pool"/>
    <rdfs:range rdf:resource="http://www.w3.org/2001/XMLSchema#string"/>
  </owl:DatatypeProperty>
</rdf:RDF>
