<?xml version="1.0" encoding="UTF-8"?>
<rdf:RDF
  xmlns:rdf="http://www.w3.org/1999/02/22-rdf-syntax-ns#"
  xmlns:rdfs="http://www.w3.org/2000/01/rdf-schema#"
  xmlns:owl="http://www.w3.org/2002/07/owl#"
  xmlns:xsd="http://www.w3.org/2001/XMLSchema#"
  xml:base="http://example.org/onto/">
  <owl:Class rdf:about="http://example.org/onto/class/google_chronicle_retrohunt">
    <rdfs:label>google_chronicle_retrohunt</rdfs:label>
    <rdfs:comment>#
#     ***     AUTO GENERATED CODE    ***    Type: MMv1     ***
#
# ----------------------------------------------------------------------------
#
#     This code is generated by Magic Modules using the following:
#
#     Configuration: https:#github.com/GoogleCloudPlatform/magic-modules/tree/main/mmv1/products/chronicle/Retrohunt.yaml
#     Template:      https:#github.com/GoogleCloudPlatform/magic-modules/tree/main/mmv1/templates/terraform/resource.html.markdown.tmpl
#
#     DO NOT EDIT this file directly. Any changes made to this file will be
#     overwritten during the next generation cycle.
#
# ----------------------------------------------------------------------------
subcategory: "Chronicle"
description: |-
  Retrohunt is an execution of a Rule over a time range in the past.
---</rdfs:comment>
  </owl:Class>
  <owl:DatatypeProperty rdf:about="http://example.org/onto/prop/google_chronicle_retrohunt_execution_interval">
    <rdfs:label>execution_interval</rdfs:label>
    <rdfs:comment>Represents a time interval, encoded as a Timestamp start (inclusive) and a
Timestamp end (exclusive).

The start must be less than or equal to the end.
When the start equals the end, the interval is empty (matches no time).
When both start and end are unspecified, the interval matches any time.</rdfs:comment>
    <rdfs:domain rdf:resource="http://example.org/onto/class/google_chronicle_retrohunt"/>
    <rdfs:range rdf:resource="http://www.w3.org/2001/XMLSchema#string"/>
  </owl:DatatypeProperty>
  <owl:DatatypeProperty rdf:about="http://example.org/onto/prop/google_chronicle_retrohunt_id">
    <rdfs:label>id</rdfs:label>
    <rdfs:domain rdf:resource="http://example.org/onto/class/google_chronicle_retrohunt"/>
    <rdfs:range rdf:resource="http://www.w3.org/2001/XMLSchema#string"/>
  </owl:DatatypeProperty>
  <owl:DatatypeProperty rdf:about="http://example.org/onto/prop/google_chronicle_retrohunt_instance">
    <rdfs:label>instance</rdfs:label>
    <rdfs:comment>The unique identifier for the Chronicle instance, which is the same as the customer ID.</rdfs:comment>
    <rdfs:domain rdf:resource="http://example.org/onto/class/google_chronicle_retrohunt"/>
    <rdfs:range rdf:resource="http://www.w3.org/2001/XMLSchema#string"/>
  </owl:DatatypeProperty>
  <owl:DatatypeProperty rdf:about="http://example.org/onto/prop/google_chronicle_retrohunt_location">
    <rdfs:label>location</rdfs:label>
    <rdfs:comment>The location of the resource. This is the geographical region where the Chronicle instance resides, such as "us" or "europe-west2".</rdfs:comment>
    <rdfs:domain rdf:resource="http://example.org/onto/class/google_chronicle_retrohunt"/>
    <rdfs:range rdf:resource="http://www.w3.org/2001/XMLSchema#string"/>
  </owl:DatatypeProperty>
  <owl:DatatypeProperty rdf:about="http://example.org/onto/prop/google_chronicle_retrohunt_name">
    <rdfs:label>name</rdfs:label>
    <rdfs:comment>The resource name of the retrohunt.
Retrohunt is the child of a rule revision. {rule} in the format below is
structured as {rule_id@revision_id}.
Format:
projects/{project}/locations/{location}/instances/{instance}/rules/{rule}/retrohunts/{retrohunt}</rdfs:comment>
    <rdfs:domain rdf:resource="http://example.org/onto/class/google_chronicle_retrohunt"/>
    <rdfs:range rdf:resource="http://www.w3.org/2001/XMLSchema#string"/>
  </owl:DatatypeProperty>
  <owl:DatatypeProperty rdf:about="http://example.org/onto/prop/google_chronicle_retrohunt_progress_percentage">
    <rdfs:label>progress_percentage</rdfs:label>
    <rdfs:comment>Output only. Percent progress of the retrohunt towards completion, from 0.00 to 100.00.</rdfs:comment>
    <rdfs:domain rdf:resource="http://example.org/onto/class/google_chronicle_retrohunt"/>
    <rdfs:range rdf:resource="http://www.w3.org/2001/XMLSchema#string"/>
  </owl:DatatypeProperty>
  <owl:DatatypeProperty rdf:about="http://example.org/onto/prop/google_chronicle_retrohunt_project">
    <rdfs:label>project</rdfs:label>
    <rdfs:domain rdf:resource="http://example.org/onto/class/google_chronicle_retrohunt"/>
    <rdfs:range rdf:resource="http://www.w3.org/2001/XMLSchema#string"/>
  </owl:DatatypeProperty>
  <owl:DatatypeProperty rdf:about="http://example.org/onto/prop/google_chronicle_retrohunt_retrohunt">
    <rdfs:label>retrohunt</rdfs:label>
    <rdfs:comment>The retrohunt ID of the Retrohunt. A retrohunt is an execution of a Rule over a time range in the past.</rdfs:comment>
    <rdfs:domain rdf:resource="http://example.org/onto/class/google_chronicle_retrohunt"/>
    <rdfs:range rdf:resource="http://www.w3.org/2001/XMLSchema#string"/>
  </owl:DatatypeProperty>
  <owl:DatatypeProperty rdf:about="http://example.org/onto/prop/google_chronicle_retrohunt_rule">
    <rdfs:label>rule</rdfs:label>
    <rdfs:comment>The Rule ID of the rule.</rdfs:comment>
    <rdfs:domain rdf:resource="http://example.org/onto/class/google_chronicle_retrohunt"/>
    <rdfs:range rdf:resource="http://www.w3.org/2001/XMLSchema#string"/>
  </owl:DatatypeProperty>
  <owl:DatatypeProperty rdf:about="http://example.org/onto/prop/google_chronicle_retrohunt_state">
    <rdfs:label>state</rdfs:label>
    <rdfs:comment>Output only. The state of the retrohunt.
Possible values:
RUNNING
DONE
CANCELLED
FAILED</rdfs:comment>
    <rdfs:domain rdf:resource="http://example.org/onto/class/google_chronicle_retrohunt"/>
    <rdfs:range rdf:resource="http://www.w3.org/2001/XMLSchema#string"/>
  </owl:DatatypeProperty>
  <owl:DatatypeProperty rdf:about="http://example.org/onto/prop/google_chronicle_retrohunt_end_time">
    <rdfs:label>end_time</rdfs:label>
    <rdfs:comment>Exclusive end of the interval.</rdfs:comment>
    <rdfs:domain rdf:resource="http://example.org/onto/class/google_chronicle_retrohunt"/>
    <rdfs:range rdf:resource="http://www.w3.org/2001/XMLSchema#string"/>
  </owl:DatatypeProperty>
  <owl:DatatypeProperty rdf:about="http://example.org/onto/prop/google_chronicle_retrohunt_start_time">
    <rdfs:label>start_time</rdfs:label>
    <rdfs:comment>Inclusive start of the interval.</rdfs:comment>
    <rdfs:domain rdf:resource="http://example.org/onto/class/google_chronicle_retrohunt"/>
    <rdfs:range rdf:resource="http://www.w3.org/2001/XMLSchema#string"/>
  </owl:DatatypeProperty>
  <owl:DatatypeProperty rdf:about="http://example.org/onto/prop/google_chronicle_retrohunt_create">
    <rdfs:label>create</rdfs:label>
    <rdfs:domain rdf:resource="http://example.org/onto/class/google_chronicle_retrohunt"/>
    <rdfs:range rdf:resource="http://www.w3.org/2001/XMLSchema#string"/>
  </owl:DatatypeProperty>
  <owl:DatatypeProperty rdf:about="http://example.org/onto/prop/google_chronicle_retrohunt_delete">
    <rdfs:label>delete</rdfs:label>
    <rdfs:domain rdf:resource="http://example.org/onto/class/google_chronicle_retrohunt"/>
    <rdfs:range rdf:resource="http://www.w3.org/2001/XMLSchema#string"/>
  </owl:DatatypeProperty>
</rdf:RDF>
