<?xml version="1.0" encoding="UTF-8"?>
<rdf:RDF
  xmlns:rdf="http://www.w3.org/1999/02/22-rdf-syntax-ns#"
  xmlns:rdfs="http://www.w3.org/2000/01/rdf-schema#"
  xmlns:owl="http://www.w3.org/2002/07/owl#"
  xmlns:xsd="http://www.w3.org/2001/XMLSchema#"
  xml:base="http://example.org/onto/">
  <owl:Class rdf:about="http://example.org/onto/class/google_cloud_tasks_queue">
    <rdfs:label>google_cloud_tasks_queue</rdfs:label>
    <rdfs:comment>#
#     ***     AUTO GENERATED CODE    ***    Type: MMv1     ***
#
# ----------------------------------------------------------------------------
#
#     This code is generated by Magic Modules using the following:
#
#     Configuration: https:#github.com/GoogleCloudPlatform/magic-modules/tree/main/mmv1/products/cloudtasks/Queue.yaml
#     Template:      https:#github.com/GoogleCloudPlatform/magic-modules/tree/main/mmv1/templates/terraform/resource.html.markdown.tmpl
#
#     DO NOT EDIT this file directly. Any changes made to this file will be
#     overwritten during the next generation cycle.
#
# ----------------------------------------------------------------------------
subcategory: "Cloud Tasks"
description: |-
  A named resource to which messages are sent by publishers.
---</rdfs:comment>
  </owl:Class>
  <owl:DatatypeProperty rdf:about="http://example.org/onto/prop/google_cloud_tasks_queue_desired_state">
    <rdfs:label>desired_state</rdfs:label>
    <rdfs:comment>The desired state of the queue. Use this to pause and resume the queue.

* RUNNING: The queue is running. Tasks can be dispatched.
* PAUSED: The queue is paused. Tasks are not dispatched but can be added to the queue. Default value: "RUNNING" Possible values: ["RUNNING", "PAUSED"]</rdfs:comment>
    <rdfs:domain rdf:resource="http://example.org/onto/class/google_cloud_tasks_queue"/>
    <rdfs:range rdf:resource="http://www.w3.org/2001/XMLSchema#string"/>
  </owl:DatatypeProperty>
  <owl:DatatypeProperty rdf:about="http://example.org/onto/prop/google_cloud_tasks_queue_id">
    <rdfs:label>id</rdfs:label>
    <rdfs:domain rdf:resource="http://example.org/onto/class/google_cloud_tasks_queue"/>
    <rdfs:range rdf:resource="http://www.w3.org/2001/XMLSchema#string"/>
  </owl:DatatypeProperty>
  <owl:DatatypeProperty rdf:about="http://example.org/onto/prop/google_cloud_tasks_queue_location">
    <rdfs:label>location</rdfs:label>
    <rdfs:comment>The location of the queue</rdfs:comment>
    <rdfs:domain rdf:resource="http://example.org/onto/class/google_cloud_tasks_queue"/>
    <rdfs:range rdf:resource="http://www.w3.org/2001/XMLSchema#string"/>
  </owl:DatatypeProperty>
  <owl:DatatypeProperty rdf:about="http://example.org/onto/prop/google_cloud_tasks_queue_name">
    <rdfs:label>name</rdfs:label>
    <rdfs:comment>The queue name.</rdfs:comment>
    <rdfs:domain rdf:resource="http://example.org/onto/class/google_cloud_tasks_queue"/>
    <rdfs:range rdf:resource="http://www.w3.org/2001/XMLSchema#string"/>
  </owl:DatatypeProperty>
  <owl:DatatypeProperty rdf:about="http://example.org/onto/prop/google_cloud_tasks_queue_project">
    <rdfs:label>project</rdfs:label>
    <rdfs:domain rdf:resource="http://example.org/onto/class/google_cloud_tasks_queue"/>
    <rdfs:range rdf:resource="http://www.w3.org/2001/XMLSchema#string"/>
  </owl:DatatypeProperty>
  <owl:DatatypeProperty rdf:about="http://example.org/onto/prop/google_cloud_tasks_queue_state">
    <rdfs:label>state</rdfs:label>
    <rdfs:comment>The current state of the queue.</rdfs:comment>
    <rdfs:domain rdf:resource="http://example.org/onto/class/google_cloud_tasks_queue"/>
    <rdfs:range rdf:resource="http://www.w3.org/2001/XMLSchema#string"/>
  </owl:DatatypeProperty>
  <owl:DatatypeProperty rdf:about="http://example.org/onto/prop/google_cloud_tasks_queue_host">
    <rdfs:label>host</rdfs:label>
    <rdfs:comment>The host that the task is sent to.</rdfs:comment>
    <rdfs:domain rdf:resource="http://example.org/onto/class/google_cloud_tasks_queue"/>
    <rdfs:range rdf:resource="http://www.w3.org/2001/XMLSchema#string"/>
  </owl:DatatypeProperty>
  <owl:DatatypeProperty rdf:about="http://example.org/onto/prop/google_cloud_tasks_queue_instance">
    <rdfs:label>instance</rdfs:label>
    <rdfs:comment>App instance.

By default, the task is sent to an instance which is available when the task is attempted.</rdfs:comment>
    <rdfs:domain rdf:resource="http://example.org/onto/class/google_cloud_tasks_queue"/>
    <rdfs:range rdf:resource="http://www.w3.org/2001/XMLSchema#string"/>
  </owl:DatatypeProperty>
  <owl:DatatypeProperty rdf:about="http://example.org/onto/prop/google_cloud_tasks_queue_service">
    <rdfs:label>service</rdfs:label>
    <rdfs:comment>App service.

By default, the task is sent to the service which is the default service when the task is attempted.</rdfs:comment>
    <rdfs:domain rdf:resource="http://example.org/onto/class/google_cloud_tasks_queue"/>
    <rdfs:range rdf:resource="http://www.w3.org/2001/XMLSchema#string"/>
  </owl:DatatypeProperty>
  <owl:DatatypeProperty rdf:about="http://example.org/onto/prop/google_cloud_tasks_queue_version">
    <rdfs:label>version</rdfs:label>
    <rdfs:comment>App version.

By default, the task is sent to the version which is the default version when the task is attempted.</rdfs:comment>
    <rdfs:domain rdf:resource="http://example.org/onto/class/google_cloud_tasks_queue"/>
    <rdfs:range rdf:resource="http://www.w3.org/2001/XMLSchema#string"/>
  </owl:DatatypeProperty>
  <owl:DatatypeProperty rdf:about="http://example.org/onto/prop/google_cloud_tasks_queue_http_method">
    <rdfs:label>http_method</rdfs:label>
    <rdfs:comment>The HTTP method to use for the request.

When specified, it overrides HttpRequest for the task.
Note that if the value is set to GET the body of the task will be ignored at execution time. Possible values: ["HTTP_METHOD_UNSPECIFIED", "POST", "GET", "HEAD", "PUT", "DELETE", "PATCH", "OPTIONS"]</rdfs:comment>
    <rdfs:domain rdf:resource="http://example.org/onto/class/google_cloud_tasks_queue"/>
    <rdfs:range rdf:resource="http://www.w3.org/2001/XMLSchema#string"/>
  </owl:DatatypeProperty>
  <owl:DatatypeProperty rdf:about="http://example.org/onto/prop/google_cloud_tasks_queue_key">
    <rdfs:label>key</rdfs:label>
    <rdfs:comment>The Key of the header.</rdfs:comment>
    <rdfs:domain rdf:resource="http://example.org/onto/class/google_cloud_tasks_queue"/>
    <rdfs:range rdf:resource="http://www.w3.org/2001/XMLSchema#string"/>
  </owl:DatatypeProperty>
  <owl:DatatypeProperty rdf:about="http://example.org/onto/prop/google_cloud_tasks_queue_value">
    <rdfs:label>value</rdfs:label>
    <rdfs:comment>The Value of the header.</rdfs:comment>
    <rdfs:domain rdf:resource="http://example.org/onto/class/google_cloud_tasks_queue"/>
    <rdfs:range rdf:resource="http://www.w3.org/2001/XMLSchema#string"/>
  </owl:DatatypeProperty>
  <owl:DatatypeProperty rdf:about="http://example.org/onto/prop/google_cloud_tasks_queue_scope">
    <rdfs:label>scope</rdfs:label>
    <rdfs:comment>OAuth scope to be used for generating OAuth access token.
If not specified, "https://www.googleapis.com/auth/cloud-platform" will be used.</rdfs:comment>
    <rdfs:domain rdf:resource="http://example.org/onto/class/google_cloud_tasks_queue"/>
    <rdfs:range rdf:resource="http://www.w3.org/2001/XMLSchema#string"/>
  </owl:DatatypeProperty>
  <owl:DatatypeProperty rdf:about="http://example.org/onto/prop/google_cloud_tasks_queue_service_account_email">
    <rdfs:label>service_account_email</rdfs:label>
    <rdfs:comment>Service account email to be used for generating OAuth token.
The service account must be within the same project as the queue.
The caller must have iam.serviceAccounts.actAs permission for the service account.</rdfs:comment>
    <rdfs:domain rdf:resource="http://example.org/onto/class/google_cloud_tasks_queue"/>
    <rdfs:range rdf:resource="http://www.w3.org/2001/XMLSchema#string"/>
  </owl:DatatypeProperty>
  <owl:DatatypeProperty rdf:about="http://example.org/onto/prop/google_cloud_tasks_queue_audience">
    <rdfs:label>audience</rdfs:label>
    <rdfs:comment>Audience to be used when generating OIDC token. If not specified, the URI specified in target will be used.</rdfs:comment>
    <rdfs:domain rdf:resource="http://example.org/onto/class/google_cloud_tasks_queue"/>
    <rdfs:range rdf:resource="http://www.w3.org/2001/XMLSchema#string"/>
  </owl:DatatypeProperty>
  <owl:DatatypeProperty rdf:about="http://example.org/onto/prop/google_cloud_tasks_queue_service_account_email">
    <rdfs:label>service_account_email</rdfs:label>
    <rdfs:comment>Service account email to be used for generating OIDC token.
The service account must be within the same project as the queue.
The caller must have iam.serviceAccounts.actAs permission for the service account.</rdfs:comment>
    <rdfs:domain rdf:resource="http://example.org/onto/class/google_cloud_tasks_queue"/>
    <rdfs:range rdf:resource="http://www.w3.org/2001/XMLSchema#string"/>
  </owl:DatatypeProperty>
  <owl:DatatypeProperty rdf:about="http://example.org/onto/prop/google_cloud_tasks_queue_host">
    <rdfs:label>host</rdfs:label>
    <rdfs:comment>Host override.

When specified, replaces the host part of the task URL.
For example, if the task URL is "https://www.google.com", and host value
is set to "example.net", the overridden URI will be changed to "https://example.net".
Host value cannot be an empty string (INVALID_ARGUMENT).</rdfs:comment>
    <rdfs:domain rdf:resource="http://example.org/onto/class/google_cloud_tasks_queue"/>
    <rdfs:range rdf:resource="http://www.w3.org/2001/XMLSchema#string"/>
  </owl:DatatypeProperty>
  <owl:DatatypeProperty rdf:about="http://example.org/onto/prop/google_cloud_tasks_queue_port">
    <rdfs:label>port</rdfs:label>
    <rdfs:comment>Port override.

When specified, replaces the port part of the task URI.
For instance, for a URI http://www.google.com/foo and port=123, the overridden URI becomes http://www.google.com:123/foo.
Note that the port value must be a positive integer.
Setting the port to 0 (Zero) clears the URI port.</rdfs:comment>
    <rdfs:domain rdf:resource="http://example.org/onto/class/google_cloud_tasks_queue"/>
    <rdfs:range rdf:resource="http://www.w3.org/2001/XMLSchema#string"/>
  </owl:DatatypeProperty>
  <owl:DatatypeProperty rdf:about="http://example.org/onto/prop/google_cloud_tasks_queue_scheme">
    <rdfs:label>scheme</rdfs:label>
    <rdfs:comment>Scheme override.

When specified, the task URI scheme is replaced by the provided value (HTTP or HTTPS). Possible values: ["HTTP", "HTTPS"]</rdfs:comment>
    <rdfs:domain rdf:resource="http://example.org/onto/class/google_cloud_tasks_queue"/>
    <rdfs:range rdf:resource="http://www.w3.org/2001/XMLSchema#string"/>
  </owl:DatatypeProperty>
  <owl:DatatypeProperty rdf:about="http://example.org/onto/prop/google_cloud_tasks_queue_uri_override_enforce_mode">
    <rdfs:label>uri_override_enforce_mode</rdfs:label>
    <rdfs:comment>URI Override Enforce Mode

When specified, determines the Target UriOverride mode. If not specified, it defaults to ALWAYS. Possible values: ["ALWAYS", "IF_NOT_EXISTS"]</rdfs:comment>
    <rdfs:domain rdf:resource="http://example.org/onto/class/google_cloud_tasks_queue"/>
    <rdfs:range rdf:resource="http://www.w3.org/2001/XMLSchema#string"/>
  </owl:DatatypeProperty>
  <owl:DatatypeProperty rdf:about="http://example.org/onto/prop/google_cloud_tasks_queue_path">
    <rdfs:label>path</rdfs:label>
    <rdfs:comment>The URI path (e.g., /users/1234). Default is an empty string.</rdfs:comment>
    <rdfs:domain rdf:resource="http://example.org/onto/class/google_cloud_tasks_queue"/>
    <rdfs:range rdf:resource="http://www.w3.org/2001/XMLSchema#string"/>
  </owl:DatatypeProperty>
  <owl:DatatypeProperty rdf:about="http://example.org/onto/prop/google_cloud_tasks_queue_query_params">
    <rdfs:label>query_params</rdfs:label>
    <rdfs:comment>The query parameters (e.g., qparam1=123&qparam2=456). Default is an empty string.</rdfs:comment>
    <rdfs:domain rdf:resource="http://example.org/onto/class/google_cloud_tasks_queue"/>
    <rdfs:range rdf:resource="http://www.w3.org/2001/XMLSchema#string"/>
  </owl:DatatypeProperty>
  <owl:DatatypeProperty rdf:about="http://example.org/onto/prop/google_cloud_tasks_queue_max_burst_size">
    <rdfs:label>max_burst_size</rdfs:label>
    <rdfs:comment>The max burst size.

Max burst size limits how fast tasks in queue are processed when many tasks are
in the queue and the rate is high. This field allows the queue to have a high
rate so processing starts shortly after a task is enqueued, but still limits
resource usage when many tasks are enqueued in a short period of time.</rdfs:comment>
    <rdfs:domain rdf:resource="http://example.org/onto/class/google_cloud_tasks_queue"/>
    <rdfs:range rdf:resource="http://www.w3.org/2001/XMLSchema#string"/>
  </owl:DatatypeProperty>
  <owl:DatatypeProperty rdf:about="http://example.org/onto/prop/google_cloud_tasks_queue_max_concurrent_dispatches">
    <rdfs:label>max_concurrent_dispatches</rdfs:label>
    <rdfs:comment>The maximum number of concurrent tasks that Cloud Tasks allows to
be dispatched for this queue. After this threshold has been
reached, Cloud Tasks stops dispatching tasks until the number of
concurrent requests decreases.</rdfs:comment>
    <rdfs:domain rdf:resource="http://example.org/onto/class/google_cloud_tasks_queue"/>
    <rdfs:range rdf:resource="http://www.w3.org/2001/XMLSchema#string"/>
  </owl:DatatypeProperty>
  <owl:DatatypeProperty rdf:about="http://example.org/onto/prop/google_cloud_tasks_queue_max_dispatches_per_second">
    <rdfs:label>max_dispatches_per_second</rdfs:label>
    <rdfs:comment>The maximum rate at which tasks are dispatched from this queue.

If unspecified when the queue is created, Cloud Tasks will pick the default.</rdfs:comment>
    <rdfs:domain rdf:resource="http://example.org/onto/class/google_cloud_tasks_queue"/>
    <rdfs:range rdf:resource="http://www.w3.org/2001/XMLSchema#string"/>
  </owl:DatatypeProperty>
  <owl:DatatypeProperty rdf:about="http://example.org/onto/prop/google_cloud_tasks_queue_max_attempts">
    <rdfs:label>max_attempts</rdfs:label>
    <rdfs:comment>Number of attempts per task.

Cloud Tasks will attempt the task maxAttempts times (that is, if
the first attempt fails, then there will be maxAttempts - 1
retries). Must be >= -1.

If unspecified when the queue is created, Cloud Tasks will pick
the default.

-1 indicates unlimited attempts.</rdfs:comment>
    <rdfs:domain rdf:resource="http://example.org/onto/class/google_cloud_tasks_queue"/>
    <rdfs:range rdf:resource="http://www.w3.org/2001/XMLSchema#string"/>
  </owl:DatatypeProperty>
  <owl:DatatypeProperty rdf:about="http://example.org/onto/prop/google_cloud_tasks_queue_max_backoff">
    <rdfs:label>max_backoff</rdfs:label>
    <rdfs:comment>A task will be scheduled for retry between minBackoff and
maxBackoff duration after it fails, if the queue's RetryConfig
specifies that the task should be retried.</rdfs:comment>
    <rdfs:domain rdf:resource="http://example.org/onto/class/google_cloud_tasks_queue"/>
    <rdfs:range rdf:resource="http://www.w3.org/2001/XMLSchema#string"/>
  </owl:DatatypeProperty>
  <owl:DatatypeProperty rdf:about="http://example.org/onto/prop/google_cloud_tasks_queue_max_doublings">
    <rdfs:label>max_doublings</rdfs:label>
    <rdfs:comment>The time between retries will double maxDoublings times.

A task's retry interval starts at minBackoff, then doubles maxDoublings times,
then increases linearly, and finally retries retries at intervals of maxBackoff
up to maxAttempts times.</rdfs:comment>
    <rdfs:domain rdf:resource="http://example.org/onto/class/google_cloud_tasks_queue"/>
    <rdfs:range rdf:resource="http://www.w3.org/2001/XMLSchema#string"/>
  </owl:DatatypeProperty>
  <owl:DatatypeProperty rdf:about="http://example.org/onto/prop/google_cloud_tasks_queue_max_retry_duration">
    <rdfs:label>max_retry_duration</rdfs:label>
    <rdfs:comment>If positive, maxRetryDuration specifies the time limit for
retrying a failed task, measured from when the task was first
attempted. Once maxRetryDuration time has passed and the task has
been attempted maxAttempts times, no further attempts will be
made and the task will be deleted.

If zero, then the task age is unlimited.</rdfs:comment>
    <rdfs:domain rdf:resource="http://example.org/onto/class/google_cloud_tasks_queue"/>
    <rdfs:range rdf:resource="http://www.w3.org/2001/XMLSchema#string"/>
  </owl:DatatypeProperty>
  <owl:DatatypeProperty rdf:about="http://example.org/onto/prop/google_cloud_tasks_queue_min_backoff">
    <rdfs:label>min_backoff</rdfs:label>
    <rdfs:comment>A task will be scheduled for retry between minBackoff and
maxBackoff duration after it fails, if the queue's RetryConfig
specifies that the task should be retried.</rdfs:comment>
    <rdfs:domain rdf:resource="http://example.org/onto/class/google_cloud_tasks_queue"/>
    <rdfs:range rdf:resource="http://www.w3.org/2001/XMLSchema#string"/>
  </owl:DatatypeProperty>
  <owl:DatatypeProperty rdf:about="http://example.org/onto/prop/google_cloud_tasks_queue_sampling_ratio">
    <rdfs:label>sampling_ratio</rdfs:label>
    <rdfs:comment>Specifies the fraction of operations to write to Stackdriver Logging.
This field may contain any value between 0.0 and 1.0, inclusive. 0.0 is the
default and means that no operations are logged.</rdfs:comment>
    <rdfs:domain rdf:resource="http://example.org/onto/class/google_cloud_tasks_queue"/>
    <rdfs:range rdf:resource="http://www.w3.org/2001/XMLSchema#string"/>
  </owl:DatatypeProperty>
  <owl:DatatypeProperty rdf:about="http://example.org/onto/prop/google_cloud_tasks_queue_create">
    <rdfs:label>create</rdfs:label>
    <rdfs:domain rdf:resource="http://example.org/onto/class/google_cloud_tasks_queue"/>
    <rdfs:range rdf:resource="http://www.w3.org/2001/XMLSchema#string"/>
  </owl:DatatypeProperty>
  <owl:DatatypeProperty rdf:about="http://example.org/onto/prop/google_cloud_tasks_queue_delete">
    <rdfs:label>delete</rdfs:label>
    <rdfs:domain rdf:resource="http://example.org/onto/class/google_cloud_tasks_queue"/>
    <rdfs:range rdf:resource="http://www.w3.org/2001/XMLSchema#string"/>
  </owl:DatatypeProperty>
  <owl:DatatypeProperty rdf:about="http://example.org/onto/prop/google_cloud_tasks_queue_update">
    <rdfs:label>update</rdfs:label>
    <rdfs:domain rdf:resource="http://example.org/onto/class/google_cloud_tasks_queue"/>
    <rdfs:range rdf:resource="http://www.w3.org/2001/XMLSchema#string"/>
  </owl:DatatypeProperty>
</rdf:RDF>
