<?xml version="1.0" encoding="UTF-8"?>
<rdf:RDF
  xmlns:rdf="http://www.w3.org/1999/02/22-rdf-syntax-ns#"
  xmlns:rdfs="http://www.w3.org/2000/01/rdf-schema#"
  xmlns:owl="http://www.w3.org/2002/07/owl#"
  xmlns:xsd="http://www.w3.org/2001/XMLSchema#"
  xml:base="http://example.org/onto/">
  <owl:Class rdf:about="http://example.org/onto/class/google_privateca_certificate_template">
    <rdfs:label>google_privateca_certificate_template</rdfs:label>
    <rdfs:comment>#
#     ***     AUTO GENERATED CODE    ***    Type: MMv1     ***
#
# ----------------------------------------------------------------------------
#
#     This code is generated by Magic Modules using the following:
#
#     Configuration: https:#github.com/GoogleCloudPlatform/magic-modules/tree/main/mmv1/products/privateca/CertificateTemplate.yaml
#     Template:      https:#github.com/GoogleCloudPlatform/magic-modules/tree/main/mmv1/templates/terraform/resource.html.markdown.tmpl
#
#     DO NOT EDIT this file directly. Any changes made to this file will be
#     overwritten during the next generation cycle.
#
# ----------------------------------------------------------------------------
subcategory: "Certificate Authority Service"
description: |-
  Certificate Authority Service provides reusable and parameterized templates that you can use for common certificate issuance scenarios.
---</rdfs:comment>
  </owl:Class>
  <owl:DatatypeProperty rdf:about="http://example.org/onto/prop/google_privateca_certificate_template_create_time">
    <rdfs:label>create_time</rdfs:label>
    <rdfs:comment>Output only. The time at which this CertificateTemplate was created.</rdfs:comment>
    <rdfs:domain rdf:resource="http://example.org/onto/class/google_privateca_certificate_template"/>
    <rdfs:range rdf:resource="http://www.w3.org/2001/XMLSchema#string"/>
  </owl:DatatypeProperty>
  <owl:DatatypeProperty rdf:about="http://example.org/onto/prop/google_privateca_certificate_template_description">
    <rdfs:label>description</rdfs:label>
    <rdfs:comment>Optional. A human-readable description of scenarios this template is intended for.</rdfs:comment>
    <rdfs:domain rdf:resource="http://example.org/onto/class/google_privateca_certificate_template"/>
    <rdfs:range rdf:resource="http://www.w3.org/2001/XMLSchema#string"/>
  </owl:DatatypeProperty>
  <owl:DatatypeProperty rdf:about="http://example.org/onto/prop/google_privateca_certificate_template_effective_labels">
    <rdfs:label>effective_labels</rdfs:label>
    <rdfs:comment>All of labels (key/value pairs) present on the resource in GCP, including the labels configured through Terraform, other clients and services.</rdfs:comment>
    <rdfs:domain rdf:resource="http://example.org/onto/class/google_privateca_certificate_template"/>
    <rdfs:range rdf:resource="http://www.w3.org/2001/XMLSchema#string"/>
  </owl:DatatypeProperty>
  <owl:DatatypeProperty rdf:about="http://example.org/onto/prop/google_privateca_certificate_template_id">
    <rdfs:label>id</rdfs:label>
    <rdfs:domain rdf:resource="http://example.org/onto/class/google_privateca_certificate_template"/>
    <rdfs:range rdf:resource="http://www.w3.org/2001/XMLSchema#string"/>
  </owl:DatatypeProperty>
  <owl:DatatypeProperty rdf:about="http://example.org/onto/prop/google_privateca_certificate_template_labels">
    <rdfs:label>labels</rdfs:label>
    <rdfs:comment>Optional. Labels with user-defined metadata.

**Note**: This field is non-authoritative, and will only manage the labels present in your configuration.
Please refer to the field 'effective_labels' for all of the labels present on the resource.</rdfs:comment>
    <rdfs:domain rdf:resource="http://example.org/onto/class/google_privateca_certificate_template"/>
    <rdfs:range rdf:resource="http://www.w3.org/2001/XMLSchema#string"/>
  </owl:DatatypeProperty>
  <owl:DatatypeProperty rdf:about="http://example.org/onto/prop/google_privateca_certificate_template_location">
    <rdfs:label>location</rdfs:label>
    <rdfs:comment>The location for the resource</rdfs:comment>
    <rdfs:domain rdf:resource="http://example.org/onto/class/google_privateca_certificate_template"/>
    <rdfs:range rdf:resource="http://www.w3.org/2001/XMLSchema#string"/>
  </owl:DatatypeProperty>
  <owl:DatatypeProperty rdf:about="http://example.org/onto/prop/google_privateca_certificate_template_maximum_lifetime">
    <rdfs:label>maximum_lifetime</rdfs:label>
    <rdfs:comment>Optional. The maximum lifetime allowed for all issued certificates that use this template. If the issuing CaPool's IssuancePolicy specifies a maximum lifetime the minimum of the two durations will be the maximum lifetime for issued. Note that if the issuing CertificateAuthority expires before a Certificate's requested maximum_lifetime, the effective lifetime will be explicitly truncated to match it.</rdfs:comment>
    <rdfs:domain rdf:resource="http://example.org/onto/class/google_privateca_certificate_template"/>
    <rdfs:range rdf:resource="http://www.w3.org/2001/XMLSchema#string"/>
  </owl:DatatypeProperty>
  <owl:DatatypeProperty rdf:about="http://example.org/onto/prop/google_privateca_certificate_template_name">
    <rdfs:label>name</rdfs:label>
    <rdfs:comment>The resource name for this CertificateTemplate in the format 'projects/*/locations/*/certificateTemplates/*'.</rdfs:comment>
    <rdfs:domain rdf:resource="http://example.org/onto/class/google_privateca_certificate_template"/>
    <rdfs:range rdf:resource="http://www.w3.org/2001/XMLSchema#string"/>
  </owl:DatatypeProperty>
  <owl:DatatypeProperty rdf:about="http://example.org/onto/prop/google_privateca_certificate_template_project">
    <rdfs:label>project</rdfs:label>
    <rdfs:domain rdf:resource="http://example.org/onto/class/google_privateca_certificate_template"/>
    <rdfs:range rdf:resource="http://www.w3.org/2001/XMLSchema#string"/>
  </owl:DatatypeProperty>
  <owl:DatatypeProperty rdf:about="http://example.org/onto/prop/google_privateca_certificate_template_terraform_labels">
    <rdfs:label>terraform_labels</rdfs:label>
    <rdfs:comment>The combination of labels configured directly on the resource
 and default labels configured on the provider.</rdfs:comment>
    <rdfs:domain rdf:resource="http://example.org/onto/class/google_privateca_certificate_template"/>
    <rdfs:range rdf:resource="http://www.w3.org/2001/XMLSchema#string"/>
  </owl:DatatypeProperty>
  <owl:DatatypeProperty rdf:about="http://example.org/onto/prop/google_privateca_certificate_template_update_time">
    <rdfs:label>update_time</rdfs:label>
    <rdfs:comment>Output only. The time at which this CertificateTemplate was updated.</rdfs:comment>
    <rdfs:domain rdf:resource="http://example.org/onto/class/google_privateca_certificate_template"/>
    <rdfs:range rdf:resource="http://www.w3.org/2001/XMLSchema#string"/>
  </owl:DatatypeProperty>
  <owl:DatatypeProperty rdf:about="http://example.org/onto/prop/google_privateca_certificate_template_allow_subject_alt_names_passthrough">
    <rdfs:label>allow_subject_alt_names_passthrough</rdfs:label>
    <rdfs:comment>Required. If this is true, the SubjectAltNames extension may be copied from a certificate request into the signed certificate. Otherwise, the requested SubjectAltNames will be discarded.</rdfs:comment>
    <rdfs:domain rdf:resource="http://example.org/onto/class/google_privateca_certificate_template"/>
    <rdfs:range rdf:resource="http://www.w3.org/2001/XMLSchema#string"/>
  </owl:DatatypeProperty>
  <owl:DatatypeProperty rdf:about="http://example.org/onto/prop/google_privateca_certificate_template_allow_subject_passthrough">
    <rdfs:label>allow_subject_passthrough</rdfs:label>
    <rdfs:comment>Required. If this is true, the Subject field may be copied from a certificate request into the signed certificate. Otherwise, the requested Subject will be discarded.</rdfs:comment>
    <rdfs:domain rdf:resource="http://example.org/onto/class/google_privateca_certificate_template"/>
    <rdfs:range rdf:resource="http://www.w3.org/2001/XMLSchema#string"/>
  </owl:DatatypeProperty>
  <owl:DatatypeProperty rdf:about="http://example.org/onto/prop/google_privateca_certificate_template_description">
    <rdfs:label>description</rdfs:label>
    <rdfs:comment>Optional. Description of the expression. This is a longer text which describes the expression, e.g. when hovered over it in a UI.</rdfs:comment>
    <rdfs:domain rdf:resource="http://example.org/onto/class/google_privateca_certificate_template"/>
    <rdfs:range rdf:resource="http://www.w3.org/2001/XMLSchema#string"/>
  </owl:DatatypeProperty>
  <owl:DatatypeProperty rdf:about="http://example.org/onto/prop/google_privateca_certificate_template_expression">
    <rdfs:label>expression</rdfs:label>
    <rdfs:comment>Textual representation of an expression in Common Expression Language syntax.</rdfs:comment>
    <rdfs:domain rdf:resource="http://example.org/onto/class/google_privateca_certificate_template"/>
    <rdfs:range rdf:resource="http://www.w3.org/2001/XMLSchema#string"/>
  </owl:DatatypeProperty>
  <owl:DatatypeProperty rdf:about="http://example.org/onto/prop/google_privateca_certificate_template_location">
    <rdfs:label>location</rdfs:label>
    <rdfs:comment>Optional. String indicating the location of the expression for error reporting, e.g. a file name and a position in the file.</rdfs:comment>
    <rdfs:domain rdf:resource="http://example.org/onto/class/google_privateca_certificate_template"/>
    <rdfs:range rdf:resource="http://www.w3.org/2001/XMLSchema#string"/>
  </owl:DatatypeProperty>
  <owl:DatatypeProperty rdf:about="http://example.org/onto/prop/google_privateca_certificate_template_title">
    <rdfs:label>title</rdfs:label>
    <rdfs:comment>Optional. Title for the expression, i.e. a short string describing its purpose. This can be used e.g. in UIs which allow to enter the expression.</rdfs:comment>
    <rdfs:domain rdf:resource="http://example.org/onto/class/google_privateca_certificate_template"/>
    <rdfs:range rdf:resource="http://www.w3.org/2001/XMLSchema#string"/>
  </owl:DatatypeProperty>
  <owl:DatatypeProperty rdf:about="http://example.org/onto/prop/google_privateca_certificate_template_known_extensions">
    <rdfs:label>known_extensions</rdfs:label>
    <rdfs:comment>Optional. A set of named X.509 extensions. Will be combined with additional_extensions to determine the full set of X.509 extensions.</rdfs:comment>
    <rdfs:domain rdf:resource="http://example.org/onto/class/google_privateca_certificate_template"/>
    <rdfs:range rdf:resource="http://www.w3.org/2001/XMLSchema#string"/>
  </owl:DatatypeProperty>
  <owl:DatatypeProperty rdf:about="http://example.org/onto/prop/google_privateca_certificate_template_object_id_path">
    <rdfs:label>object_id_path</rdfs:label>
    <rdfs:comment>Required. The parts of an OID path. The most significant parts of the path come first.</rdfs:comment>
    <rdfs:domain rdf:resource="http://example.org/onto/class/google_privateca_certificate_template"/>
    <rdfs:range rdf:resource="http://www.w3.org/2001/XMLSchema#string"/>
  </owl:DatatypeProperty>
  <owl:DatatypeProperty rdf:about="http://example.org/onto/prop/google_privateca_certificate_template_aia_ocsp_servers">
    <rdfs:label>aia_ocsp_servers</rdfs:label>
    <rdfs:comment>Optional. Describes Online Certificate Status Protocol (OCSP) endpoint addresses that appear in the "Authority Information Access" extension in the certificate.</rdfs:comment>
    <rdfs:domain rdf:resource="http://example.org/onto/class/google_privateca_certificate_template"/>
    <rdfs:range rdf:resource="http://www.w3.org/2001/XMLSchema#string"/>
  </owl:DatatypeProperty>
  <owl:DatatypeProperty rdf:about="http://example.org/onto/prop/google_privateca_certificate_template_critical">
    <rdfs:label>critical</rdfs:label>
    <rdfs:comment>Optional. Indicates whether or not this extension is critical (i.e., if the client does not know how to handle this extension, the client should consider this to be an error).</rdfs:comment>
    <rdfs:domain rdf:resource="http://example.org/onto/class/google_privateca_certificate_template"/>
    <rdfs:range rdf:resource="http://www.w3.org/2001/XMLSchema#string"/>
  </owl:DatatypeProperty>
  <owl:DatatypeProperty rdf:about="http://example.org/onto/prop/google_privateca_certificate_template_value">
    <rdfs:label>value</rdfs:label>
    <rdfs:comment>Required. The value of this X.509 extension.</rdfs:comment>
    <rdfs:domain rdf:resource="http://example.org/onto/class/google_privateca_certificate_template"/>
    <rdfs:range rdf:resource="http://www.w3.org/2001/XMLSchema#string"/>
  </owl:DatatypeProperty>
  <owl:DatatypeProperty rdf:about="http://example.org/onto/prop/google_privateca_certificate_template_object_id_path">
    <rdfs:label>object_id_path</rdfs:label>
    <rdfs:comment>Required. The parts of an OID path. The most significant parts of the path come first.</rdfs:comment>
    <rdfs:domain rdf:resource="http://example.org/onto/class/google_privateca_certificate_template"/>
    <rdfs:range rdf:resource="http://www.w3.org/2001/XMLSchema#string"/>
  </owl:DatatypeProperty>
  <owl:DatatypeProperty rdf:about="http://example.org/onto/prop/google_privateca_certificate_template_is_ca">
    <rdfs:label>is_ca</rdfs:label>
    <rdfs:comment>Optional. Refers to the "CA" X.509 extension, which is a boolean value. When this value is true, the "CA" in Basic Constraints extension will be set to true.</rdfs:comment>
    <rdfs:domain rdf:resource="http://example.org/onto/class/google_privateca_certificate_template"/>
    <rdfs:range rdf:resource="http://www.w3.org/2001/XMLSchema#string"/>
  </owl:DatatypeProperty>
  <owl:DatatypeProperty rdf:about="http://example.org/onto/prop/google_privateca_certificate_template_max_issuer_path_length">
    <rdfs:label>max_issuer_path_length</rdfs:label>
    <rdfs:comment>Optional. Refers to the "path length constraint" in Basic Constraints extension. For a CA certificate, this value describes the depth of
subordinate CA certificates that are allowed. If this value is less than 0, the request will fail.</rdfs:comment>
    <rdfs:domain rdf:resource="http://example.org/onto/class/google_privateca_certificate_template"/>
    <rdfs:range rdf:resource="http://www.w3.org/2001/XMLSchema#string"/>
  </owl:DatatypeProperty>
  <owl:DatatypeProperty rdf:about="http://example.org/onto/prop/google_privateca_certificate_template_null_ca">
    <rdfs:label>null_ca</rdfs:label>
    <rdfs:comment>Optional. When true, the "CA" in Basic Constraints extension will be set to null and omitted from the CA certificate.
If both 'is_ca' and 'null_ca' are unset, the "CA" in Basic Constraints extension will be set to false.
Note that the behavior when 'is_ca = false' for this resource is different from the behavior in the Certificate Authority, Certificate and CaPool resources.</rdfs:comment>
    <rdfs:domain rdf:resource="http://example.org/onto/class/google_privateca_certificate_template"/>
    <rdfs:range rdf:resource="http://www.w3.org/2001/XMLSchema#string"/>
  </owl:DatatypeProperty>
  <owl:DatatypeProperty rdf:about="http://example.org/onto/prop/google_privateca_certificate_template_zero_max_issuer_path_length">
    <rdfs:label>zero_max_issuer_path_length</rdfs:label>
    <rdfs:comment>Optional. When true, the "path length constraint" in Basic Constraints extension will be set to 0.
if both 'max_issuer_path_length' and 'zero_max_issuer_path_length' are unset,
the max path length will be omitted from the CA certificate.</rdfs:comment>
    <rdfs:domain rdf:resource="http://example.org/onto/class/google_privateca_certificate_template"/>
    <rdfs:range rdf:resource="http://www.w3.org/2001/XMLSchema#string"/>
  </owl:DatatypeProperty>
  <owl:DatatypeProperty rdf:about="http://example.org/onto/prop/google_privateca_certificate_template_cert_sign">
    <rdfs:label>cert_sign</rdfs:label>
    <rdfs:comment>The key may be used to sign certificates.</rdfs:comment>
    <rdfs:domain rdf:resource="http://example.org/onto/class/google_privateca_certificate_template"/>
    <rdfs:range rdf:resource="http://www.w3.org/2001/XMLSchema#string"/>
  </owl:DatatypeProperty>
  <owl:DatatypeProperty rdf:about="http://example.org/onto/prop/google_privateca_certificate_template_content_commitment">
    <rdfs:label>content_commitment</rdfs:label>
    <rdfs:comment>The key may be used for cryptographic commitments. Note that this may also be referred to as "non-repudiation".</rdfs:comment>
    <rdfs:domain rdf:resource="http://example.org/onto/class/google_privateca_certificate_template"/>
    <rdfs:range rdf:resource="http://www.w3.org/2001/XMLSchema#string"/>
  </owl:DatatypeProperty>
  <owl:DatatypeProperty rdf:about="http://example.org/onto/prop/google_privateca_certificate_template_crl_sign">
    <rdfs:label>crl_sign</rdfs:label>
    <rdfs:comment>The key may be used sign certificate revocation lists.</rdfs:comment>
    <rdfs:domain rdf:resource="http://example.org/onto/class/google_privateca_certificate_template"/>
    <rdfs:range rdf:resource="http://www.w3.org/2001/XMLSchema#string"/>
  </owl:DatatypeProperty>
  <owl:DatatypeProperty rdf:about="http://example.org/onto/prop/google_privateca_certificate_template_data_encipherment">
    <rdfs:label>data_encipherment</rdfs:label>
    <rdfs:comment>The key may be used to encipher data.</rdfs:comment>
    <rdfs:domain rdf:resource="http://example.org/onto/class/google_privateca_certificate_template"/>
    <rdfs:range rdf:resource="http://www.w3.org/2001/XMLSchema#string"/>
  </owl:DatatypeProperty>
  <owl:DatatypeProperty rdf:about="http://example.org/onto/prop/google_privateca_certificate_template_decipher_only">
    <rdfs:label>decipher_only</rdfs:label>
    <rdfs:comment>The key may be used to decipher only.</rdfs:comment>
    <rdfs:domain rdf:resource="http://example.org/onto/class/google_privateca_certificate_template"/>
    <rdfs:range rdf:resource="http://www.w3.org/2001/XMLSchema#string"/>
  </owl:DatatypeProperty>
  <owl:DatatypeProperty rdf:about="http://example.org/onto/prop/google_privateca_certificate_template_digital_signature">
    <rdfs:label>digital_signature</rdfs:label>
    <rdfs:comment>The key may be used for digital signatures.</rdfs:comment>
    <rdfs:domain rdf:resource="http://example.org/onto/class/google_privateca_certificate_template"/>
    <rdfs:range rdf:resource="http://www.w3.org/2001/XMLSchema#string"/>
  </owl:DatatypeProperty>
  <owl:DatatypeProperty rdf:about="http://example.org/onto/prop/google_privateca_certificate_template_encipher_only">
    <rdfs:label>encipher_only</rdfs:label>
    <rdfs:comment>The key may be used to encipher only.</rdfs:comment>
    <rdfs:domain rdf:resource="http://example.org/onto/class/google_privateca_certificate_template"/>
    <rdfs:range rdf:resource="http://www.w3.org/2001/XMLSchema#string"/>
  </owl:DatatypeProperty>
  <owl:DatatypeProperty rdf:about="http://example.org/onto/prop/google_privateca_certificate_template_key_agreement">
    <rdfs:label>key_agreement</rdfs:label>
    <rdfs:comment>The key may be used in a key agreement protocol.</rdfs:comment>
    <rdfs:domain rdf:resource="http://example.org/onto/class/google_privateca_certificate_template"/>
    <rdfs:range rdf:resource="http://www.w3.org/2001/XMLSchema#string"/>
  </owl:DatatypeProperty>
  <owl:DatatypeProperty rdf:about="http://example.org/onto/prop/google_privateca_certificate_template_key_encipherment">
    <rdfs:label>key_encipherment</rdfs:label>
    <rdfs:comment>The key may be used to encipher other keys.</rdfs:comment>
    <rdfs:domain rdf:resource="http://example.org/onto/class/google_privateca_certificate_template"/>
    <rdfs:range rdf:resource="http://www.w3.org/2001/XMLSchema#string"/>
  </owl:DatatypeProperty>
  <owl:DatatypeProperty rdf:about="http://example.org/onto/prop/google_privateca_certificate_template_client_auth">
    <rdfs:label>client_auth</rdfs:label>
    <rdfs:comment>Corresponds to OID 1.3.6.1.5.5.7.3.2. Officially described as "TLS WWW client authentication", though regularly used for non-WWW TLS.</rdfs:comment>
    <rdfs:domain rdf:resource="http://example.org/onto/class/google_privateca_certificate_template"/>
    <rdfs:range rdf:resource="http://www.w3.org/2001/XMLSchema#string"/>
  </owl:DatatypeProperty>
  <owl:DatatypeProperty rdf:about="http://example.org/onto/prop/google_privateca_certificate_template_code_signing">
    <rdfs:label>code_signing</rdfs:label>
    <rdfs:comment>Corresponds to OID 1.3.6.1.5.5.7.3.3. Officially described as "Signing of downloadable executable code client authentication".</rdfs:comment>
    <rdfs:domain rdf:resource="http://example.org/onto/class/google_privateca_certificate_template"/>
    <rdfs:range rdf:resource="http://www.w3.org/2001/XMLSchema#string"/>
  </owl:DatatypeProperty>
  <owl:DatatypeProperty rdf:about="http://example.org/onto/prop/google_privateca_certificate_template_email_protection">
    <rdfs:label>email_protection</rdfs:label>
    <rdfs:comment>Corresponds to OID 1.3.6.1.5.5.7.3.4. Officially described as "Email protection".</rdfs:comment>
    <rdfs:domain rdf:resource="http://example.org/onto/class/google_privateca_certificate_template"/>
    <rdfs:range rdf:resource="http://www.w3.org/2001/XMLSchema#string"/>
  </owl:DatatypeProperty>
  <owl:DatatypeProperty rdf:about="http://example.org/onto/prop/google_privateca_certificate_template_ocsp_signing">
    <rdfs:label>ocsp_signing</rdfs:label>
    <rdfs:comment>Corresponds to OID 1.3.6.1.5.5.7.3.9. Officially described as "Signing OCSP responses".</rdfs:comment>
    <rdfs:domain rdf:resource="http://example.org/onto/class/google_privateca_certificate_template"/>
    <rdfs:range rdf:resource="http://www.w3.org/2001/XMLSchema#string"/>
  </owl:DatatypeProperty>
  <owl:DatatypeProperty rdf:about="http://example.org/onto/prop/google_privateca_certificate_template_server_auth">
    <rdfs:label>server_auth</rdfs:label>
    <rdfs:comment>Corresponds to OID 1.3.6.1.5.5.7.3.1. Officially described as "TLS WWW server authentication", though regularly used for non-WWW TLS.</rdfs:comment>
    <rdfs:domain rdf:resource="http://example.org/onto/class/google_privateca_certificate_template"/>
    <rdfs:range rdf:resource="http://www.w3.org/2001/XMLSchema#string"/>
  </owl:DatatypeProperty>
  <owl:DatatypeProperty rdf:about="http://example.org/onto/prop/google_privateca_certificate_template_time_stamping">
    <rdfs:label>time_stamping</rdfs:label>
    <rdfs:comment>Corresponds to OID 1.3.6.1.5.5.7.3.8. Officially described as "Binding the hash of an object to a time".</rdfs:comment>
    <rdfs:domain rdf:resource="http://example.org/onto/class/google_privateca_certificate_template"/>
    <rdfs:range rdf:resource="http://www.w3.org/2001/XMLSchema#string"/>
  </owl:DatatypeProperty>
  <owl:DatatypeProperty rdf:about="http://example.org/onto/prop/google_privateca_certificate_template_object_id_path">
    <rdfs:label>object_id_path</rdfs:label>
    <rdfs:comment>Required. The parts of an OID path. The most significant parts of the path come first.</rdfs:comment>
    <rdfs:domain rdf:resource="http://example.org/onto/class/google_privateca_certificate_template"/>
    <rdfs:range rdf:resource="http://www.w3.org/2001/XMLSchema#string"/>
  </owl:DatatypeProperty>
  <owl:DatatypeProperty rdf:about="http://example.org/onto/prop/google_privateca_certificate_template_critical">
    <rdfs:label>critical</rdfs:label>
    <rdfs:comment>Indicates whether or not the name constraints are marked critical.</rdfs:comment>
    <rdfs:domain rdf:resource="http://example.org/onto/class/google_privateca_certificate_template"/>
    <rdfs:range rdf:resource="http://www.w3.org/2001/XMLSchema#string"/>
  </owl:DatatypeProperty>
  <owl:DatatypeProperty rdf:about="http://example.org/onto/prop/google_privateca_certificate_template_excluded_dns_names">
    <rdfs:label>excluded_dns_names</rdfs:label>
    <rdfs:comment>Contains excluded DNS names. Any DNS name that can be
constructed by simply adding zero or more labels to
the left-hand side of the name satisfies the name constraint.
For example, 'example.com', 'www.example.com', 'www.sub.example.com'
would satisfy 'example.com' while 'example1.com' does not.</rdfs:comment>
    <rdfs:domain rdf:resource="http://example.org/onto/class/google_privateca_certificate_template"/>
    <rdfs:range rdf:resource="http://www.w3.org/2001/XMLSchema#string"/>
  </owl:DatatypeProperty>
  <owl:DatatypeProperty rdf:about="http://example.org/onto/prop/google_privateca_certificate_template_excluded_email_addresses">
    <rdfs:label>excluded_email_addresses</rdfs:label>
    <rdfs:comment>Contains the excluded email addresses. The value can be a particular
email address, a hostname to indicate all email addresses on that host or
a domain with a leading period (e.g. '.example.com') to indicate
all email addresses in that domain.</rdfs:comment>
    <rdfs:domain rdf:resource="http://example.org/onto/class/google_privateca_certificate_template"/>
    <rdfs:range rdf:resource="http://www.w3.org/2001/XMLSchema#string"/>
  </owl:DatatypeProperty>
  <owl:DatatypeProperty rdf:about="http://example.org/onto/prop/google_privateca_certificate_template_excluded_ip_ranges">
    <rdfs:label>excluded_ip_ranges</rdfs:label>
    <rdfs:comment>Contains the excluded IP ranges. For IPv4 addresses, the ranges
are expressed using CIDR notation as specified in RFC 4632.
For IPv6 addresses, the ranges are expressed in similar encoding as IPv4
addresses.</rdfs:comment>
    <rdfs:domain rdf:resource="http://example.org/onto/class/google_privateca_certificate_template"/>
    <rdfs:range rdf:resource="http://www.w3.org/2001/XMLSchema#string"/>
  </owl:DatatypeProperty>
  <owl:DatatypeProperty rdf:about="http://example.org/onto/prop/google_privateca_certificate_template_excluded_uris">
    <rdfs:label>excluded_uris</rdfs:label>
    <rdfs:comment>Contains the excluded URIs that apply to the host part of the name.
The value can be a hostname or a domain with a
leading period (like '.example.com')</rdfs:comment>
    <rdfs:domain rdf:resource="http://example.org/onto/class/google_privateca_certificate_template"/>
    <rdfs:range rdf:resource="http://www.w3.org/2001/XMLSchema#string"/>
  </owl:DatatypeProperty>
  <owl:DatatypeProperty rdf:about="http://example.org/onto/prop/google_privateca_certificate_template_permitted_dns_names">
    <rdfs:label>permitted_dns_names</rdfs:label>
    <rdfs:comment>Contains permitted DNS names. Any DNS name that can be
constructed by simply adding zero or more labels to
the left-hand side of the name satisfies the name constraint.
For example, 'example.com', 'www.example.com', 'www.sub.example.com'
would satisfy 'example.com' while 'example1.com' does not.</rdfs:comment>
    <rdfs:domain rdf:resource="http://example.org/onto/class/google_privateca_certificate_template"/>
    <rdfs:range rdf:resource="http://www.w3.org/2001/XMLSchema#string"/>
  </owl:DatatypeProperty>
  <owl:DatatypeProperty rdf:about="http://example.org/onto/prop/google_privateca_certificate_template_permitted_email_addresses">
    <rdfs:label>permitted_email_addresses</rdfs:label>
    <rdfs:comment>Contains the permitted email addresses. The value can be a particular
email address, a hostname to indicate all email addresses on that host or
a domain with a leading period (e.g. '.example.com') to indicate
all email addresses in that domain.</rdfs:comment>
    <rdfs:domain rdf:resource="http://example.org/onto/class/google_privateca_certificate_template"/>
    <rdfs:range rdf:resource="http://www.w3.org/2001/XMLSchema#string"/>
  </owl:DatatypeProperty>
  <owl:DatatypeProperty rdf:about="http://example.org/onto/prop/google_privateca_certificate_template_permitted_ip_ranges">
    <rdfs:label>permitted_ip_ranges</rdfs:label>
    <rdfs:comment>Contains the permitted IP ranges. For IPv4 addresses, the ranges
are expressed using CIDR notation as specified in RFC 4632.
For IPv6 addresses, the ranges are expressed in similar encoding as IPv4
addresses.</rdfs:comment>
    <rdfs:domain rdf:resource="http://example.org/onto/class/google_privateca_certificate_template"/>
    <rdfs:range rdf:resource="http://www.w3.org/2001/XMLSchema#string"/>
  </owl:DatatypeProperty>
  <owl:DatatypeProperty rdf:about="http://example.org/onto/prop/google_privateca_certificate_template_permitted_uris">
    <rdfs:label>permitted_uris</rdfs:label>
    <rdfs:comment>Contains the permitted URIs that apply to the host part of the name.
The value can be a hostname or a domain with a
leading period (like '.example.com')</rdfs:comment>
    <rdfs:domain rdf:resource="http://example.org/onto/class/google_privateca_certificate_template"/>
    <rdfs:range rdf:resource="http://www.w3.org/2001/XMLSchema#string"/>
  </owl:DatatypeProperty>
  <owl:DatatypeProperty rdf:about="http://example.org/onto/prop/google_privateca_certificate_template_object_id_path">
    <rdfs:label>object_id_path</rdfs:label>
    <rdfs:comment>Required. The parts of an OID path. The most significant parts of the path come first.</rdfs:comment>
    <rdfs:domain rdf:resource="http://example.org/onto/class/google_privateca_certificate_template"/>
    <rdfs:range rdf:resource="http://www.w3.org/2001/XMLSchema#string"/>
  </owl:DatatypeProperty>
  <owl:DatatypeProperty rdf:about="http://example.org/onto/prop/google_privateca_certificate_template_create">
    <rdfs:label>create</rdfs:label>
    <rdfs:domain rdf:resource="http://example.org/onto/class/google_privateca_certificate_template"/>
    <rdfs:range rdf:resource="http://www.w3.org/2001/XMLSchema#string"/>
  </owl:DatatypeProperty>
  <owl:DatatypeProperty rdf:about="http://example.org/onto/prop/google_privateca_certificate_template_delete">
    <rdfs:label>delete</rdfs:label>
    <rdfs:domain rdf:resource="http://example.org/onto/class/google_privateca_certificate_template"/>
    <rdfs:range rdf:resource="http://www.w3.org/2001/XMLSchema#string"/>
  </owl:DatatypeProperty>
  <owl:DatatypeProperty rdf:about="http://example.org/onto/prop/google_privateca_certificate_template_update">
    <rdfs:label>update</rdfs:label>
    <rdfs:domain rdf:resource="http://example.org/onto/class/google_privateca_certificate_template"/>
    <rdfs:range rdf:resource="http://www.w3.org/2001/XMLSchema#string"/>
  </owl:DatatypeProperty>
</rdf:RDF>
