<?xml version="1.0" encoding="UTF-8"?>
<rdf:RDF
  xmlns:rdf="http://www.w3.org/1999/02/22-rdf-syntax-ns#"
  xmlns:rdfs="http://www.w3.org/2000/01/rdf-schema#"
  xmlns:owl="http://www.w3.org/2002/07/owl#"
  xmlns:xsd="http://www.w3.org/2001/XMLSchema#"
  xml:base="http://example.org/onto/">
  <owl:Class rdf:about="http://example.org/onto/class/google_dialogflow_cx_flow">
    <rdfs:label>google_dialogflow_cx_flow</rdfs:label>
    <rdfs:comment>#
#     ***     AUTO GENERATED CODE    ***    Type: MMv1     ***
#
# ----------------------------------------------------------------------------
#
#     This code is generated by Magic Modules using the following:
#
#     Configuration: https:#github.com/GoogleCloudPlatform/magic-modules/tree/main/mmv1/products/dialogflowcx/Flow.yaml
#     Template:      https:#github.com/GoogleCloudPlatform/magic-modules/tree/main/mmv1/templates/terraform/resource.html.markdown.tmpl
#
#     DO NOT EDIT this file directly. Any changes made to this file will be
#     overwritten during the next generation cycle.
#
# ----------------------------------------------------------------------------
subcategory: "Dialogflow CX"
description: |-
  Flows represents the conversation flows when you build your chatbot agent.
---</rdfs:comment>
  </owl:Class>
  <owl:DatatypeProperty rdf:about="http://example.org/onto/prop/google_dialogflow_cx_flow_description">
    <rdfs:label>description</rdfs:label>
    <rdfs:comment>The description of the flow. The maximum length is 500 characters. If exceeded, the request is rejected.</rdfs:comment>
    <rdfs:domain rdf:resource="http://example.org/onto/class/google_dialogflow_cx_flow"/>
    <rdfs:range rdf:resource="http://www.w3.org/2001/XMLSchema#string"/>
  </owl:DatatypeProperty>
  <owl:DatatypeProperty rdf:about="http://example.org/onto/prop/google_dialogflow_cx_flow_display_name">
    <rdfs:label>display_name</rdfs:label>
    <rdfs:comment>The human-readable name of the flow.</rdfs:comment>
    <rdfs:domain rdf:resource="http://example.org/onto/class/google_dialogflow_cx_flow"/>
    <rdfs:range rdf:resource="http://www.w3.org/2001/XMLSchema#string"/>
  </owl:DatatypeProperty>
  <owl:DatatypeProperty rdf:about="http://example.org/onto/prop/google_dialogflow_cx_flow_id">
    <rdfs:label>id</rdfs:label>
    <rdfs:domain rdf:resource="http://example.org/onto/class/google_dialogflow_cx_flow"/>
    <rdfs:range rdf:resource="http://www.w3.org/2001/XMLSchema#string"/>
  </owl:DatatypeProperty>
  <owl:DatatypeProperty rdf:about="http://example.org/onto/prop/google_dialogflow_cx_flow_is_default_start_flow">
    <rdfs:label>is_default_start_flow</rdfs:label>
    <rdfs:comment>Marks this as the [Default Start Flow](https://cloud.google.com/dialogflow/cx/docs/concept/flow#start) for an agent. When you create an agent, the Default Start Flow is created automatically.
The Default Start Flow cannot be deleted; deleting the 'google_dialogflow_cx_flow' resource does nothing to the underlying GCP resources.

~> Avoid having multiple 'google_dialogflow_cx_flow' resources linked to the same agent with 'is_default_start_flow = true' because they will compete to control a single Default Start Flow resource in GCP.</rdfs:comment>
    <rdfs:domain rdf:resource="http://example.org/onto/class/google_dialogflow_cx_flow"/>
    <rdfs:range rdf:resource="http://www.w3.org/2001/XMLSchema#string"/>
  </owl:DatatypeProperty>
  <owl:DatatypeProperty rdf:about="http://example.org/onto/prop/google_dialogflow_cx_flow_language_code">
    <rdfs:label>language_code</rdfs:label>
    <rdfs:comment>The language of the following fields in flow:
Flow.event_handlers.trigger_fulfillment.messages
Flow.event_handlers.trigger_fulfillment.conditional_cases
Flow.transition_routes.trigger_fulfillment.messages
Flow.transition_routes.trigger_fulfillment.conditional_cases
If not specified, the agent's default language is used. Many languages are supported. Note: languages must be enabled in the agent before they can be used.</rdfs:comment>
    <rdfs:domain rdf:resource="http://example.org/onto/class/google_dialogflow_cx_flow"/>
    <rdfs:range rdf:resource="http://www.w3.org/2001/XMLSchema#string"/>
  </owl:DatatypeProperty>
  <owl:DatatypeProperty rdf:about="http://example.org/onto/prop/google_dialogflow_cx_flow_name">
    <rdfs:label>name</rdfs:label>
    <rdfs:comment>The unique identifier of the flow.
Format: projects/<Project ID>/locations/<Location ID>/agents/<Agent ID>/flows/<Flow ID>.</rdfs:comment>
    <rdfs:domain rdf:resource="http://example.org/onto/class/google_dialogflow_cx_flow"/>
    <rdfs:range rdf:resource="http://www.w3.org/2001/XMLSchema#string"/>
  </owl:DatatypeProperty>
  <owl:DatatypeProperty rdf:about="http://example.org/onto/prop/google_dialogflow_cx_flow_parent">
    <rdfs:label>parent</rdfs:label>
    <rdfs:comment>The agent to create a flow for.
Format: projects/<Project ID>/locations/<Location ID>/agents/<Agent ID>.</rdfs:comment>
    <rdfs:domain rdf:resource="http://example.org/onto/class/google_dialogflow_cx_flow"/>
    <rdfs:range rdf:resource="http://www.w3.org/2001/XMLSchema#string"/>
  </owl:DatatypeProperty>
  <owl:DatatypeProperty rdf:about="http://example.org/onto/prop/google_dialogflow_cx_flow_transition_route_groups">
    <rdfs:label>transition_route_groups</rdfs:label>
    <rdfs:comment>A flow's transition route group serve two purposes:
They are responsible for matching the user's first utterances in the flow.
They are inherited by every page's [transition route groups][Page.transition_route_groups]. Transition route groups defined in the page have higher priority than those defined in the flow.
Format:projects/<Project ID>/locations/<Location ID>/agents/<Agent ID>/flows/<Flow ID>/transitionRouteGroups/<TransitionRouteGroup ID>.</rdfs:comment>
    <rdfs:domain rdf:resource="http://example.org/onto/class/google_dialogflow_cx_flow"/>
    <rdfs:range rdf:resource="http://www.w3.org/2001/XMLSchema#string"/>
  </owl:DatatypeProperty>
  <owl:DatatypeProperty rdf:about="http://example.org/onto/prop/google_dialogflow_cx_flow_uri">
    <rdfs:label>uri</rdfs:label>
    <rdfs:comment>The Google Cloud Storage URI for the exported objects. Whether a full object name, or just a prefix, its usage depends on the Dialogflow operation.
Format: gs://bucket/object-name-or-prefix</rdfs:comment>
    <rdfs:domain rdf:resource="http://example.org/onto/class/google_dialogflow_cx_flow"/>
    <rdfs:range rdf:resource="http://www.w3.org/2001/XMLSchema#string"/>
  </owl:DatatypeProperty>
  <owl:DatatypeProperty rdf:about="http://example.org/onto/prop/google_dialogflow_cx_flow_enabled">
    <rdfs:label>enabled</rdfs:label>
    <rdfs:comment>If true, incoming audio is processed for DTMF (dual tone multi frequency) events. For example, if the caller presses a button on their telephone keypad and DTMF processing is enabled, Dialogflow will detect the event (e.g. a "3" was pressed) in the incoming audio and pass the event to the bot to drive business logic (e.g. when 3 is pressed, return the account balance).</rdfs:comment>
    <rdfs:domain rdf:resource="http://example.org/onto/class/google_dialogflow_cx_flow"/>
    <rdfs:range rdf:resource="http://www.w3.org/2001/XMLSchema#string"/>
  </owl:DatatypeProperty>
  <owl:DatatypeProperty rdf:about="http://example.org/onto/prop/google_dialogflow_cx_flow_finish_digit">
    <rdfs:label>finish_digit</rdfs:label>
    <rdfs:comment>The digit that terminates a DTMF digit sequence.</rdfs:comment>
    <rdfs:domain rdf:resource="http://example.org/onto/class/google_dialogflow_cx_flow"/>
    <rdfs:range rdf:resource="http://www.w3.org/2001/XMLSchema#string"/>
  </owl:DatatypeProperty>
  <owl:DatatypeProperty rdf:about="http://example.org/onto/prop/google_dialogflow_cx_flow_max_digits">
    <rdfs:label>max_digits</rdfs:label>
    <rdfs:comment>Max length of DTMF digits.</rdfs:comment>
    <rdfs:domain rdf:resource="http://example.org/onto/class/google_dialogflow_cx_flow"/>
    <rdfs:range rdf:resource="http://www.w3.org/2001/XMLSchema#string"/>
  </owl:DatatypeProperty>
  <owl:DatatypeProperty rdf:about="http://example.org/onto/prop/google_dialogflow_cx_flow_enable_consent_based_redaction">
    <rdfs:label>enable_consent_based_redaction</rdfs:label>
    <rdfs:comment>Enables consent-based end-user input redaction, if true, a pre-defined session parameter **$session.params.conversation-redaction** will be used to determine if the utterance should be redacted.</rdfs:comment>
    <rdfs:domain rdf:resource="http://example.org/onto/class/google_dialogflow_cx_flow"/>
    <rdfs:range rdf:resource="http://www.w3.org/2001/XMLSchema#string"/>
  </owl:DatatypeProperty>
  <owl:DatatypeProperty rdf:about="http://example.org/onto/prop/google_dialogflow_cx_flow_enable_interaction_logging">
    <rdfs:label>enable_interaction_logging</rdfs:label>
    <rdfs:comment>Enables DF Interaction logging.</rdfs:comment>
    <rdfs:domain rdf:resource="http://example.org/onto/class/google_dialogflow_cx_flow"/>
    <rdfs:range rdf:resource="http://www.w3.org/2001/XMLSchema#string"/>
  </owl:DatatypeProperty>
  <owl:DatatypeProperty rdf:about="http://example.org/onto/prop/google_dialogflow_cx_flow_enable_stackdriver_logging">
    <rdfs:label>enable_stackdriver_logging</rdfs:label>
    <rdfs:comment>Enables Google Cloud Logging.</rdfs:comment>
    <rdfs:domain rdf:resource="http://example.org/onto/class/google_dialogflow_cx_flow"/>
    <rdfs:range rdf:resource="http://www.w3.org/2001/XMLSchema#string"/>
  </owl:DatatypeProperty>
  <owl:DatatypeProperty rdf:about="http://example.org/onto/prop/google_dialogflow_cx_flow_endpointer_sensitivity">
    <rdfs:label>endpointer_sensitivity</rdfs:label>
    <rdfs:comment>Sensitivity of the speech model that detects the end of speech. Scale from 0 to 100.</rdfs:comment>
    <rdfs:domain rdf:resource="http://example.org/onto/class/google_dialogflow_cx_flow"/>
    <rdfs:range rdf:resource="http://www.w3.org/2001/XMLSchema#string"/>
  </owl:DatatypeProperty>
  <owl:DatatypeProperty rdf:about="http://example.org/onto/prop/google_dialogflow_cx_flow_models">
    <rdfs:label>models</rdfs:label>
    <rdfs:comment>Mapping from language to Speech-to-Text model. The mapped Speech-to-Text model will be selected for requests from its corresponding language. For more information, see [Speech models](https://cloud.google.com/dialogflow/cx/docs/concept/speech-models).
An object containing a list of **"key": value** pairs. Example: **{ "name": "wrench", "mass": "1.3kg", "count": "3" }**.</rdfs:comment>
    <rdfs:domain rdf:resource="http://example.org/onto/class/google_dialogflow_cx_flow"/>
    <rdfs:range rdf:resource="http://www.w3.org/2001/XMLSchema#string"/>
  </owl:DatatypeProperty>
  <owl:DatatypeProperty rdf:about="http://example.org/onto/prop/google_dialogflow_cx_flow_no_speech_timeout">
    <rdfs:label>no_speech_timeout</rdfs:label>
    <rdfs:comment>Timeout before detecting no speech.
A duration in seconds with up to nine fractional digits, ending with 's'. Example: "3.5s".</rdfs:comment>
    <rdfs:domain rdf:resource="http://example.org/onto/class/google_dialogflow_cx_flow"/>
    <rdfs:range rdf:resource="http://www.w3.org/2001/XMLSchema#string"/>
  </owl:DatatypeProperty>
  <owl:DatatypeProperty rdf:about="http://example.org/onto/prop/google_dialogflow_cx_flow_use_timeout_based_endpointing">
    <rdfs:label>use_timeout_based_endpointing</rdfs:label>
    <rdfs:comment>Use timeout based endpointing, interpreting endpointer sensitivity as seconds of timeout value.</rdfs:comment>
    <rdfs:domain rdf:resource="http://example.org/onto/class/google_dialogflow_cx_flow"/>
    <rdfs:range rdf:resource="http://www.w3.org/2001/XMLSchema#string"/>
  </owl:DatatypeProperty>
  <owl:DatatypeProperty rdf:about="http://example.org/onto/prop/google_dialogflow_cx_flow_event">
    <rdfs:label>event</rdfs:label>
    <rdfs:comment>The name of the event to handle.</rdfs:comment>
    <rdfs:domain rdf:resource="http://example.org/onto/class/google_dialogflow_cx_flow"/>
    <rdfs:range rdf:resource="http://www.w3.org/2001/XMLSchema#string"/>
  </owl:DatatypeProperty>
  <owl:DatatypeProperty rdf:about="http://example.org/onto/prop/google_dialogflow_cx_flow_name">
    <rdfs:label>name</rdfs:label>
    <rdfs:comment>The unique identifier of this event handler.</rdfs:comment>
    <rdfs:domain rdf:resource="http://example.org/onto/class/google_dialogflow_cx_flow"/>
    <rdfs:range rdf:resource="http://www.w3.org/2001/XMLSchema#string"/>
  </owl:DatatypeProperty>
  <owl:DatatypeProperty rdf:about="http://example.org/onto/prop/google_dialogflow_cx_flow_target_flow">
    <rdfs:label>target_flow</rdfs:label>
    <rdfs:comment>The target flow to transition to.
Format: projects/<Project ID>/locations/<Location ID>/agents/<Agent ID>/flows/<Flow ID>.</rdfs:comment>
    <rdfs:domain rdf:resource="http://example.org/onto/class/google_dialogflow_cx_flow"/>
    <rdfs:range rdf:resource="http://www.w3.org/2001/XMLSchema#string"/>
  </owl:DatatypeProperty>
  <owl:DatatypeProperty rdf:about="http://example.org/onto/prop/google_dialogflow_cx_flow_target_page">
    <rdfs:label>target_page</rdfs:label>
    <rdfs:comment>The target page to transition to.
Format: projects/<Project ID>/locations/<Location ID>/agents/<Agent ID>/flows/<Flow ID>/pages/<Page ID>.</rdfs:comment>
    <rdfs:domain rdf:resource="http://example.org/onto/class/google_dialogflow_cx_flow"/>
    <rdfs:range rdf:resource="http://www.w3.org/2001/XMLSchema#string"/>
  </owl:DatatypeProperty>
  <owl:DatatypeProperty rdf:about="http://example.org/onto/prop/google_dialogflow_cx_flow_enable_generative_fallback">
    <rdfs:label>enable_generative_fallback</rdfs:label>
    <rdfs:comment>If the flag is true, the agent will utilize LLM to generate a text response.
If LLM generation fails, the defined responses in the fulfillment will be respected.
This flag is only useful for fulfillments associated with no-match event handlers.</rdfs:comment>
    <rdfs:domain rdf:resource="http://example.org/onto/class/google_dialogflow_cx_flow"/>
    <rdfs:range rdf:resource="http://www.w3.org/2001/XMLSchema#string"/>
  </owl:DatatypeProperty>
  <owl:DatatypeProperty rdf:about="http://example.org/onto/prop/google_dialogflow_cx_flow_return_partial_responses">
    <rdfs:label>return_partial_responses</rdfs:label>
    <rdfs:comment>Whether Dialogflow should return currently queued fulfillment response messages in streaming APIs. If a webhook is specified, it happens before Dialogflow invokes webhook. Warning: 1) This flag only affects streaming API. Responses are still queued and returned once in non-streaming API. 2) The flag can be enabled in any fulfillment but only the first 3 partial responses will be returned. You may only want to apply it to fulfillments that have slow webhooks.</rdfs:comment>
    <rdfs:domain rdf:resource="http://example.org/onto/class/google_dialogflow_cx_flow"/>
    <rdfs:range rdf:resource="http://www.w3.org/2001/XMLSchema#string"/>
  </owl:DatatypeProperty>
  <owl:DatatypeProperty rdf:about="http://example.org/onto/prop/google_dialogflow_cx_flow_tag">
    <rdfs:label>tag</rdfs:label>
    <rdfs:comment>The tag used by the webhook to identify which fulfillment is being called. This field is required if webhook is specified.</rdfs:comment>
    <rdfs:domain rdf:resource="http://example.org/onto/class/google_dialogflow_cx_flow"/>
    <rdfs:range rdf:resource="http://www.w3.org/2001/XMLSchema#string"/>
  </owl:DatatypeProperty>
  <owl:DatatypeProperty rdf:about="http://example.org/onto/prop/google_dialogflow_cx_flow_webhook">
    <rdfs:label>webhook</rdfs:label>
    <rdfs:comment>The webhook to call. Format: projects/<Project ID>/locations/<Location ID>/agents/<Agent ID>/webhooks/<Webhook ID>.</rdfs:comment>
    <rdfs:domain rdf:resource="http://example.org/onto/class/google_dialogflow_cx_flow"/>
    <rdfs:range rdf:resource="http://www.w3.org/2001/XMLSchema#string"/>
  </owl:DatatypeProperty>
  <owl:DatatypeProperty rdf:about="http://example.org/onto/prop/google_dialogflow_cx_flow_cases">
    <rdfs:label>cases</rdfs:label>
    <rdfs:comment>A JSON encoded list of cascading if-else conditions. Cases are mutually exclusive. The first one with a matching condition is selected, all the rest ignored.
See [Case](https://cloud.google.com/dialogflow/cx/docs/reference/rest/v3/Fulfillment#case) for the schema.</rdfs:comment>
    <rdfs:domain rdf:resource="http://example.org/onto/class/google_dialogflow_cx_flow"/>
    <rdfs:range rdf:resource="http://www.w3.org/2001/XMLSchema#string"/>
  </owl:DatatypeProperty>
  <owl:DatatypeProperty rdf:about="http://example.org/onto/prop/google_dialogflow_cx_flow_channel">
    <rdfs:label>channel</rdfs:label>
    <rdfs:comment>The channel which the response is associated with. Clients can specify the channel via QueryParameters.channel, and only associated channel response will be returned.</rdfs:comment>
    <rdfs:domain rdf:resource="http://example.org/onto/class/google_dialogflow_cx_flow"/>
    <rdfs:range rdf:resource="http://www.w3.org/2001/XMLSchema#string"/>
  </owl:DatatypeProperty>
  <owl:DatatypeProperty rdf:about="http://example.org/onto/prop/google_dialogflow_cx_flow_payload">
    <rdfs:label>payload</rdfs:label>
    <rdfs:comment>A custom, platform-specific payload.</rdfs:comment>
    <rdfs:domain rdf:resource="http://example.org/onto/class/google_dialogflow_cx_flow"/>
    <rdfs:range rdf:resource="http://www.w3.org/2001/XMLSchema#string"/>
  </owl:DatatypeProperty>
  <owl:DatatypeProperty rdf:about="http://example.org/onto/prop/google_dialogflow_cx_flow_metadata">
    <rdfs:label>metadata</rdfs:label>
    <rdfs:comment>Custom metadata. Dialogflow doesn't impose any structure on this.</rdfs:comment>
    <rdfs:domain rdf:resource="http://example.org/onto/class/google_dialogflow_cx_flow"/>
    <rdfs:range rdf:resource="http://www.w3.org/2001/XMLSchema#string"/>
  </owl:DatatypeProperty>
  <owl:DatatypeProperty rdf:about="http://example.org/onto/prop/google_dialogflow_cx_flow_metadata">
    <rdfs:label>metadata</rdfs:label>
    <rdfs:comment>Custom metadata. Dialogflow doesn't impose any structure on this.</rdfs:comment>
    <rdfs:domain rdf:resource="http://example.org/onto/class/google_dialogflow_cx_flow"/>
    <rdfs:range rdf:resource="http://www.w3.org/2001/XMLSchema#string"/>
  </owl:DatatypeProperty>
  <owl:DatatypeProperty rdf:about="http://example.org/onto/prop/google_dialogflow_cx_flow_allow_playback_interruption">
    <rdfs:label>allow_playback_interruption</rdfs:label>
    <rdfs:comment>Whether the playback of this message can be interrupted by the end user's speech and the client can then starts the next Dialogflow request.</rdfs:comment>
    <rdfs:domain rdf:resource="http://example.org/onto/class/google_dialogflow_cx_flow"/>
    <rdfs:range rdf:resource="http://www.w3.org/2001/XMLSchema#string"/>
  </owl:DatatypeProperty>
  <owl:DatatypeProperty rdf:about="http://example.org/onto/prop/google_dialogflow_cx_flow_ssml">
    <rdfs:label>ssml</rdfs:label>
    <rdfs:comment>The SSML text to be synthesized. For more information, see SSML.</rdfs:comment>
    <rdfs:domain rdf:resource="http://example.org/onto/class/google_dialogflow_cx_flow"/>
    <rdfs:range rdf:resource="http://www.w3.org/2001/XMLSchema#string"/>
  </owl:DatatypeProperty>
  <owl:DatatypeProperty rdf:about="http://example.org/onto/prop/google_dialogflow_cx_flow_text">
    <rdfs:label>text</rdfs:label>
    <rdfs:comment>The raw text to be synthesized.</rdfs:comment>
    <rdfs:domain rdf:resource="http://example.org/onto/class/google_dialogflow_cx_flow"/>
    <rdfs:range rdf:resource="http://www.w3.org/2001/XMLSchema#string"/>
  </owl:DatatypeProperty>
  <owl:DatatypeProperty rdf:about="http://example.org/onto/prop/google_dialogflow_cx_flow_allow_playback_interruption">
    <rdfs:label>allow_playback_interruption</rdfs:label>
    <rdfs:comment>Whether the playback of this message can be interrupted by the end user's speech and the client can then starts the next Dialogflow request.</rdfs:comment>
    <rdfs:domain rdf:resource="http://example.org/onto/class/google_dialogflow_cx_flow"/>
    <rdfs:range rdf:resource="http://www.w3.org/2001/XMLSchema#string"/>
  </owl:DatatypeProperty>
  <owl:DatatypeProperty rdf:about="http://example.org/onto/prop/google_dialogflow_cx_flow_audio_uri">
    <rdfs:label>audio_uri</rdfs:label>
    <rdfs:comment>URI of the audio clip. Dialogflow does not impose any validation on this value. It is specific to the client that reads it.</rdfs:comment>
    <rdfs:domain rdf:resource="http://example.org/onto/class/google_dialogflow_cx_flow"/>
    <rdfs:range rdf:resource="http://www.w3.org/2001/XMLSchema#string"/>
  </owl:DatatypeProperty>
  <owl:DatatypeProperty rdf:about="http://example.org/onto/prop/google_dialogflow_cx_flow_phone_number">
    <rdfs:label>phone_number</rdfs:label>
    <rdfs:comment>Transfer the call to a phone number in E.164 format.</rdfs:comment>
    <rdfs:domain rdf:resource="http://example.org/onto/class/google_dialogflow_cx_flow"/>
    <rdfs:range rdf:resource="http://www.w3.org/2001/XMLSchema#string"/>
  </owl:DatatypeProperty>
  <owl:DatatypeProperty rdf:about="http://example.org/onto/prop/google_dialogflow_cx_flow_allow_playback_interruption">
    <rdfs:label>allow_playback_interruption</rdfs:label>
    <rdfs:comment>Whether the playback of this message can be interrupted by the end user's speech and the client can then starts the next Dialogflow request.</rdfs:comment>
    <rdfs:domain rdf:resource="http://example.org/onto/class/google_dialogflow_cx_flow"/>
    <rdfs:range rdf:resource="http://www.w3.org/2001/XMLSchema#string"/>
  </owl:DatatypeProperty>
  <owl:DatatypeProperty rdf:about="http://example.org/onto/prop/google_dialogflow_cx_flow_text">
    <rdfs:label>text</rdfs:label>
    <rdfs:comment>A collection of text responses.</rdfs:comment>
    <rdfs:domain rdf:resource="http://example.org/onto/class/google_dialogflow_cx_flow"/>
    <rdfs:range rdf:resource="http://www.w3.org/2001/XMLSchema#string"/>
  </owl:DatatypeProperty>
  <owl:DatatypeProperty rdf:about="http://example.org/onto/prop/google_dialogflow_cx_flow_parameter">
    <rdfs:label>parameter</rdfs:label>
    <rdfs:comment>Display name of the parameter.</rdfs:comment>
    <rdfs:domain rdf:resource="http://example.org/onto/class/google_dialogflow_cx_flow"/>
    <rdfs:range rdf:resource="http://www.w3.org/2001/XMLSchema#string"/>
  </owl:DatatypeProperty>
  <owl:DatatypeProperty rdf:about="http://example.org/onto/prop/google_dialogflow_cx_flow_value">
    <rdfs:label>value</rdfs:label>
    <rdfs:comment>The new JSON-encoded value of the parameter. A null value clears the parameter.</rdfs:comment>
    <rdfs:domain rdf:resource="http://example.org/onto/class/google_dialogflow_cx_flow"/>
    <rdfs:range rdf:resource="http://www.w3.org/2001/XMLSchema#string"/>
  </owl:DatatypeProperty>
  <owl:DatatypeProperty rdf:about="http://example.org/onto/prop/google_dialogflow_cx_flow_enabled">
    <rdfs:label>enabled</rdfs:label>
    <rdfs:comment>Whether Knowledge Connector is enabled or not.</rdfs:comment>
    <rdfs:domain rdf:resource="http://example.org/onto/class/google_dialogflow_cx_flow"/>
    <rdfs:range rdf:resource="http://www.w3.org/2001/XMLSchema#string"/>
  </owl:DatatypeProperty>
  <owl:DatatypeProperty rdf:about="http://example.org/onto/prop/google_dialogflow_cx_flow_target_flow">
    <rdfs:label>target_flow</rdfs:label>
    <rdfs:comment>The target flow to transition to. Format: projects/<ProjectID>/locations/<LocationID>/agents/<AgentID>/flows/<FlowID>.
This field is part of a union field 'target': Only one of 'targetPage' or 'targetFlow' may be set.</rdfs:comment>
    <rdfs:domain rdf:resource="http://example.org/onto/class/google_dialogflow_cx_flow"/>
    <rdfs:range rdf:resource="http://www.w3.org/2001/XMLSchema#string"/>
  </owl:DatatypeProperty>
  <owl:DatatypeProperty rdf:about="http://example.org/onto/prop/google_dialogflow_cx_flow_target_page">
    <rdfs:label>target_page</rdfs:label>
    <rdfs:comment>The target page to transition to. Format: projects/<ProjectID>/locations/<LocationID>/agents/<AgentID>/flows/<FlowID>/pages/<PageID>.
The page must be in the same host flow (the flow that owns this 'KnowledgeConnectorSettings').
This field is part of a union field 'target': Only one of 'targetPage' or 'targetFlow' may be set.</rdfs:comment>
    <rdfs:domain rdf:resource="http://example.org/onto/class/google_dialogflow_cx_flow"/>
    <rdfs:range rdf:resource="http://www.w3.org/2001/XMLSchema#string"/>
  </owl:DatatypeProperty>
  <owl:DatatypeProperty rdf:about="http://example.org/onto/prop/google_dialogflow_cx_flow_data_store">
    <rdfs:label>data_store</rdfs:label>
    <rdfs:comment>The full name of the referenced data store. Formats: projects/{project}/locations/{location}/collections/{collection}/dataStores/{dataStore} projects/{project}/locations/{location}/dataStores/{dataStore}</rdfs:comment>
    <rdfs:domain rdf:resource="http://example.org/onto/class/google_dialogflow_cx_flow"/>
    <rdfs:range rdf:resource="http://www.w3.org/2001/XMLSchema#string"/>
  </owl:DatatypeProperty>
  <owl:DatatypeProperty rdf:about="http://example.org/onto/prop/google_dialogflow_cx_flow_data_store_type">
    <rdfs:label>data_store_type</rdfs:label>
    <rdfs:comment>The type of the connected data store.
* PUBLIC_WEB: A data store that contains public web content.
* UNSTRUCTURED: A data store that contains unstructured private data.
* STRUCTURED: A data store that contains structured data (for example FAQ). Possible values: ["PUBLIC_WEB", "UNSTRUCTURED", "STRUCTURED"]</rdfs:comment>
    <rdfs:domain rdf:resource="http://example.org/onto/class/google_dialogflow_cx_flow"/>
    <rdfs:range rdf:resource="http://www.w3.org/2001/XMLSchema#string"/>
  </owl:DatatypeProperty>
  <owl:DatatypeProperty rdf:about="http://example.org/onto/prop/google_dialogflow_cx_flow_document_processing_mode">
    <rdfs:label>document_processing_mode</rdfs:label>
    <rdfs:comment>The document processing mode for the data store connection. Should only be set for PUBLIC_WEB and UNSTRUCTURED data stores. If not set it is considered as DOCUMENTS, as this is the legacy mode.
* DOCUMENTS: Documents are processed as documents.
* CHUNKS: Documents are converted to chunks. Possible values: ["DOCUMENTS", "CHUNKS"]</rdfs:comment>
    <rdfs:domain rdf:resource="http://example.org/onto/class/google_dialogflow_cx_flow"/>
    <rdfs:range rdf:resource="http://www.w3.org/2001/XMLSchema#string"/>
  </owl:DatatypeProperty>
  <owl:DatatypeProperty rdf:about="http://example.org/onto/prop/google_dialogflow_cx_flow_enable_generative_fallback">
    <rdfs:label>enable_generative_fallback</rdfs:label>
    <rdfs:comment>If the flag is true, the agent will utilize LLM to generate a text response. If LLM generation fails, the defined responses in the fulfillment will be respected. This flag is only useful for fulfillments associated with no-match event handlers.</rdfs:comment>
    <rdfs:domain rdf:resource="http://example.org/onto/class/google_dialogflow_cx_flow"/>
    <rdfs:range rdf:resource="http://www.w3.org/2001/XMLSchema#string"/>
  </owl:DatatypeProperty>
  <owl:DatatypeProperty rdf:about="http://example.org/onto/prop/google_dialogflow_cx_flow_return_partial_responses">
    <rdfs:label>return_partial_responses</rdfs:label>
    <rdfs:comment>Whether Dialogflow should return currently queued fulfillment response messages in streaming APIs. If a webhook is specified, it happens before Dialogflow invokes webhook. Warning: 1) This flag only affects streaming API. Responses are still queued and returned once in non-streaming API. 2) The flag can be enabled in any fulfillment but only the first 3 partial responses will be returned. You may only want to apply it to fulfillments that have slow webhooks.</rdfs:comment>
    <rdfs:domain rdf:resource="http://example.org/onto/class/google_dialogflow_cx_flow"/>
    <rdfs:range rdf:resource="http://www.w3.org/2001/XMLSchema#string"/>
  </owl:DatatypeProperty>
  <owl:DatatypeProperty rdf:about="http://example.org/onto/prop/google_dialogflow_cx_flow_tag">
    <rdfs:label>tag</rdfs:label>
    <rdfs:comment>The tag used by the webhook to identify which fulfillment is being called. This field is required if webhook is specified.</rdfs:comment>
    <rdfs:domain rdf:resource="http://example.org/onto/class/google_dialogflow_cx_flow"/>
    <rdfs:range rdf:resource="http://www.w3.org/2001/XMLSchema#string"/>
  </owl:DatatypeProperty>
  <owl:DatatypeProperty rdf:about="http://example.org/onto/prop/google_dialogflow_cx_flow_webhook">
    <rdfs:label>webhook</rdfs:label>
    <rdfs:comment>The webhook to call. Format: projects/<Project ID>/locations/<Location ID>/agents/<Agent ID>/webhooks/<Webhook ID>.</rdfs:comment>
    <rdfs:domain rdf:resource="http://example.org/onto/class/google_dialogflow_cx_flow"/>
    <rdfs:range rdf:resource="http://www.w3.org/2001/XMLSchema#string"/>
  </owl:DatatypeProperty>
  <owl:DatatypeProperty rdf:about="http://example.org/onto/prop/google_dialogflow_cx_flow_enabled">
    <rdfs:label>enabled</rdfs:label>
    <rdfs:comment>If true, incoming audio is processed for DTMF (dual tone multi frequtectency) events. For example, if the caller presses a button on their telephone keypad and DTMF processing is enabled, Dialogflow will de the event (e.g. a "3" was pressed) in the incoming audio and pass the event to the bot to drive business logic (e.g. when 3 is pressed, return the account balance).</rdfs:comment>
    <rdfs:domain rdf:resource="http://example.org/onto/class/google_dialogflow_cx_flow"/>
    <rdfs:range rdf:resource="http://www.w3.org/2001/XMLSchema#string"/>
  </owl:DatatypeProperty>
  <owl:DatatypeProperty rdf:about="http://example.org/onto/prop/google_dialogflow_cx_flow_endpointing_timeout_duration">
    <rdfs:label>endpointing_timeout_duration</rdfs:label>
    <rdfs:comment>Endpoint timeout setting for matching dtmf input to regex.
A duration in seconds with up to nine fractional digits, ending with 's'. Example: "3.500s".</rdfs:comment>
    <rdfs:domain rdf:resource="http://example.org/onto/class/google_dialogflow_cx_flow"/>
    <rdfs:range rdf:resource="http://www.w3.org/2001/XMLSchema#string"/>
  </owl:DatatypeProperty>
  <owl:DatatypeProperty rdf:about="http://example.org/onto/prop/google_dialogflow_cx_flow_finish_digit">
    <rdfs:label>finish_digit</rdfs:label>
    <rdfs:comment>The digit that terminates a DTMF digit sequence.</rdfs:comment>
    <rdfs:domain rdf:resource="http://example.org/onto/class/google_dialogflow_cx_flow"/>
    <rdfs:range rdf:resource="http://www.w3.org/2001/XMLSchema#string"/>
  </owl:DatatypeProperty>
  <owl:DatatypeProperty rdf:about="http://example.org/onto/prop/google_dialogflow_cx_flow_interdigit_timeout_duration">
    <rdfs:label>interdigit_timeout_duration</rdfs:label>
    <rdfs:comment>Interdigit timeout setting for matching dtmf input to regex.
A duration in seconds with up to nine fractional digits, ending with 's'. Example: "3.500s".</rdfs:comment>
    <rdfs:domain rdf:resource="http://example.org/onto/class/google_dialogflow_cx_flow"/>
    <rdfs:range rdf:resource="http://www.w3.org/2001/XMLSchema#string"/>
  </owl:DatatypeProperty>
  <owl:DatatypeProperty rdf:about="http://example.org/onto/prop/google_dialogflow_cx_flow_max_digits">
    <rdfs:label>max_digits</rdfs:label>
    <rdfs:comment>Max length of DTMF digits.</rdfs:comment>
    <rdfs:domain rdf:resource="http://example.org/onto/class/google_dialogflow_cx_flow"/>
    <rdfs:range rdf:resource="http://www.w3.org/2001/XMLSchema#string"/>
  </owl:DatatypeProperty>
  <owl:DatatypeProperty rdf:about="http://example.org/onto/prop/google_dialogflow_cx_flow_enable_consent_based_redaction">
    <rdfs:label>enable_consent_based_redaction</rdfs:label>
    <rdfs:comment>Enables consent-based end-user input redaction, if true, a pre-defined session parameter **$session.params.conversation-redaction** will be used to determine if the utterance should be redacted.</rdfs:comment>
    <rdfs:domain rdf:resource="http://example.org/onto/class/google_dialogflow_cx_flow"/>
    <rdfs:range rdf:resource="http://www.w3.org/2001/XMLSchema#string"/>
  </owl:DatatypeProperty>
  <owl:DatatypeProperty rdf:about="http://example.org/onto/prop/google_dialogflow_cx_flow_enable_interaction_logging">
    <rdfs:label>enable_interaction_logging</rdfs:label>
    <rdfs:comment>Enables DF Interaction logging.</rdfs:comment>
    <rdfs:domain rdf:resource="http://example.org/onto/class/google_dialogflow_cx_flow"/>
    <rdfs:range rdf:resource="http://www.w3.org/2001/XMLSchema#string"/>
  </owl:DatatypeProperty>
  <owl:DatatypeProperty rdf:about="http://example.org/onto/prop/google_dialogflow_cx_flow_enable_stackdriver_logging">
    <rdfs:label>enable_stackdriver_logging</rdfs:label>
    <rdfs:comment>Enables Google Cloud Logging.</rdfs:comment>
    <rdfs:domain rdf:resource="http://example.org/onto/class/google_dialogflow_cx_flow"/>
    <rdfs:range rdf:resource="http://www.w3.org/2001/XMLSchema#string"/>
  </owl:DatatypeProperty>
  <owl:DatatypeProperty rdf:about="http://example.org/onto/prop/google_dialogflow_cx_flow_endpointer_sensitivity">
    <rdfs:label>endpointer_sensitivity</rdfs:label>
    <rdfs:comment>Sensitivity of the speech model that detects the end of speech. Scale from 0 to 100.</rdfs:comment>
    <rdfs:domain rdf:resource="http://example.org/onto/class/google_dialogflow_cx_flow"/>
    <rdfs:range rdf:resource="http://www.w3.org/2001/XMLSchema#string"/>
  </owl:DatatypeProperty>
  <owl:DatatypeProperty rdf:about="http://example.org/onto/prop/google_dialogflow_cx_flow_models">
    <rdfs:label>models</rdfs:label>
    <rdfs:comment>Mapping from language to Speech-to-Text model. The mapped Speech-to-Text model will be selected for requests from its corresponding language. For more information, see [Speech models](https://cloud.google.com/dialogflow/cx/docs/concept/speech-models).
An object containing a list of **"key": value** pairs. Example: **{ "name": "wrench", "mass": "1.3kg", "count": "3" }**.</rdfs:comment>
    <rdfs:domain rdf:resource="http://example.org/onto/class/google_dialogflow_cx_flow"/>
    <rdfs:range rdf:resource="http://www.w3.org/2001/XMLSchema#string"/>
  </owl:DatatypeProperty>
  <owl:DatatypeProperty rdf:about="http://example.org/onto/prop/google_dialogflow_cx_flow_no_speech_timeout">
    <rdfs:label>no_speech_timeout</rdfs:label>
    <rdfs:comment>Timeout before detecting no speech.
A duration in seconds with up to nine fractional digits, ending with 's'. Example: "3.500s".</rdfs:comment>
    <rdfs:domain rdf:resource="http://example.org/onto/class/google_dialogflow_cx_flow"/>
    <rdfs:range rdf:resource="http://www.w3.org/2001/XMLSchema#string"/>
  </owl:DatatypeProperty>
  <owl:DatatypeProperty rdf:about="http://example.org/onto/prop/google_dialogflow_cx_flow_use_timeout_based_endpointing">
    <rdfs:label>use_timeout_based_endpointing</rdfs:label>
    <rdfs:comment>Use timeout based endpointing, interpreting endpointer sensitivity as seconds of timeout value.</rdfs:comment>
    <rdfs:domain rdf:resource="http://example.org/onto/class/google_dialogflow_cx_flow"/>
    <rdfs:range rdf:resource="http://www.w3.org/2001/XMLSchema#string"/>
  </owl:DatatypeProperty>
  <owl:DatatypeProperty rdf:about="http://example.org/onto/prop/google_dialogflow_cx_flow_cases">
    <rdfs:label>cases</rdfs:label>
    <rdfs:comment>A JSON encoded list of cascading if-else conditions. Cases are mutually exclusive. The first one with a matching condition is selected, all the rest ignored.
See [Case](https://cloud.google.com/dialogflow/cx/docs/reference/rest/v3/Fulfillment#case) for the schema.</rdfs:comment>
    <rdfs:domain rdf:resource="http://example.org/onto/class/google_dialogflow_cx_flow"/>
    <rdfs:range rdf:resource="http://www.w3.org/2001/XMLSchema#string"/>
  </owl:DatatypeProperty>
  <owl:DatatypeProperty rdf:about="http://example.org/onto/prop/google_dialogflow_cx_flow_channel">
    <rdfs:label>channel</rdfs:label>
    <rdfs:comment>The channel which the response is associated with. Clients can specify the channel via QueryParameters.channel, and only associated channel response will be returned.</rdfs:comment>
    <rdfs:domain rdf:resource="http://example.org/onto/class/google_dialogflow_cx_flow"/>
    <rdfs:range rdf:resource="http://www.w3.org/2001/XMLSchema#string"/>
  </owl:DatatypeProperty>
  <owl:DatatypeProperty rdf:about="http://example.org/onto/prop/google_dialogflow_cx_flow_end_interaction">
    <rdfs:label>end_interaction</rdfs:label>
    <rdfs:comment>This type has no fields.
Indicates that interaction with the Dialogflow agent has ended. This message is generated by Dialogflow only and not supposed to be defined by the user.
This field is part of a union field 'message': Only one of 'text', 'payload', 'conversationSuccess', 'outputAudioText', 'liveAgentHandoff', 'endInteraction', 'playAudio', 'mixedAudio', 'telephonyTransferCall', or 'knowledgeInfoCard' may be set.</rdfs:comment>
    <rdfs:domain rdf:resource="http://example.org/onto/class/google_dialogflow_cx_flow"/>
    <rdfs:range rdf:resource="http://www.w3.org/2001/XMLSchema#string"/>
  </owl:DatatypeProperty>
  <owl:DatatypeProperty rdf:about="http://example.org/onto/prop/google_dialogflow_cx_flow_mixed_audio">
    <rdfs:label>mixed_audio</rdfs:label>
    <rdfs:comment>Represents an audio message that is composed of both segments synthesized from the Dialogflow agent prompts and ones hosted externally at the specified URIs. The external URIs are specified via playAudio. This message is generated by Dialogflow only and not supposed to be defined by the user.
This field is part of a union field 'message': Only one of 'text', 'payload', 'conversationSuccess', 'outputAudioText', 'liveAgentHandoff', 'endInteraction', 'playAudio', 'mixedAudio', 'telephonyTransferCall', or 'knowledgeInfoCard' may be set.</rdfs:comment>
    <rdfs:domain rdf:resource="http://example.org/onto/class/google_dialogflow_cx_flow"/>
    <rdfs:range rdf:resource="http://www.w3.org/2001/XMLSchema#string"/>
  </owl:DatatypeProperty>
  <owl:DatatypeProperty rdf:about="http://example.org/onto/prop/google_dialogflow_cx_flow_payload">
    <rdfs:label>payload</rdfs:label>
    <rdfs:comment>Returns a response containing a custom, platform-specific payload.
This field is part of a union field 'message': Only one of 'text', 'payload', 'conversationSuccess', 'outputAudioText', 'liveAgentHandoff', 'endInteraction', 'playAudio', 'mixedAudio', 'telephonyTransferCall', or 'knowledgeInfoCard' may be set.</rdfs:comment>
    <rdfs:domain rdf:resource="http://example.org/onto/class/google_dialogflow_cx_flow"/>
    <rdfs:range rdf:resource="http://www.w3.org/2001/XMLSchema#string"/>
  </owl:DatatypeProperty>
  <owl:DatatypeProperty rdf:about="http://example.org/onto/prop/google_dialogflow_cx_flow_metadata">
    <rdfs:label>metadata</rdfs:label>
    <rdfs:comment>Custom metadata. Dialogflow doesn't impose any structure on this.</rdfs:comment>
    <rdfs:domain rdf:resource="http://example.org/onto/class/google_dialogflow_cx_flow"/>
    <rdfs:range rdf:resource="http://www.w3.org/2001/XMLSchema#string"/>
  </owl:DatatypeProperty>
  <owl:DatatypeProperty rdf:about="http://example.org/onto/prop/google_dialogflow_cx_flow_metadata">
    <rdfs:label>metadata</rdfs:label>
    <rdfs:comment>Custom metadata. Dialogflow doesn't impose any structure on this.</rdfs:comment>
    <rdfs:domain rdf:resource="http://example.org/onto/class/google_dialogflow_cx_flow"/>
    <rdfs:range rdf:resource="http://www.w3.org/2001/XMLSchema#string"/>
  </owl:DatatypeProperty>
  <owl:DatatypeProperty rdf:about="http://example.org/onto/prop/google_dialogflow_cx_flow_allow_playback_interruption">
    <rdfs:label>allow_playback_interruption</rdfs:label>
    <rdfs:comment>Whether the playback of this message can be interrupted by the end user's speech and the client can then starts the next Dialogflow request.</rdfs:comment>
    <rdfs:domain rdf:resource="http://example.org/onto/class/google_dialogflow_cx_flow"/>
    <rdfs:range rdf:resource="http://www.w3.org/2001/XMLSchema#string"/>
  </owl:DatatypeProperty>
  <owl:DatatypeProperty rdf:about="http://example.org/onto/prop/google_dialogflow_cx_flow_ssml">
    <rdfs:label>ssml</rdfs:label>
    <rdfs:comment>The SSML text to be synthesized. For more information, see SSML.
This field is part of a union field 'source': Only one of 'text' or 'ssml' may be set.</rdfs:comment>
    <rdfs:domain rdf:resource="http://example.org/onto/class/google_dialogflow_cx_flow"/>
    <rdfs:range rdf:resource="http://www.w3.org/2001/XMLSchema#string"/>
  </owl:DatatypeProperty>
  <owl:DatatypeProperty rdf:about="http://example.org/onto/prop/google_dialogflow_cx_flow_text">
    <rdfs:label>text</rdfs:label>
    <rdfs:comment>The raw text to be synthesized.
This field is part of a union field 'source': Only one of 'text' or 'ssml' may be set.</rdfs:comment>
    <rdfs:domain rdf:resource="http://example.org/onto/class/google_dialogflow_cx_flow"/>
    <rdfs:range rdf:resource="http://www.w3.org/2001/XMLSchema#string"/>
  </owl:DatatypeProperty>
  <owl:DatatypeProperty rdf:about="http://example.org/onto/prop/google_dialogflow_cx_flow_allow_playback_interruption">
    <rdfs:label>allow_playback_interruption</rdfs:label>
    <rdfs:comment>Whether the playback of this message can be interrupted by the end user's speech and the client can then starts the next Dialogflow request.</rdfs:comment>
    <rdfs:domain rdf:resource="http://example.org/onto/class/google_dialogflow_cx_flow"/>
    <rdfs:range rdf:resource="http://www.w3.org/2001/XMLSchema#string"/>
  </owl:DatatypeProperty>
  <owl:DatatypeProperty rdf:about="http://example.org/onto/prop/google_dialogflow_cx_flow_audio_uri">
    <rdfs:label>audio_uri</rdfs:label>
    <rdfs:comment>URI of the audio clip. Dialogflow does not impose any validation on this value. It is specific to the client that reads it.</rdfs:comment>
    <rdfs:domain rdf:resource="http://example.org/onto/class/google_dialogflow_cx_flow"/>
    <rdfs:range rdf:resource="http://www.w3.org/2001/XMLSchema#string"/>
  </owl:DatatypeProperty>
  <owl:DatatypeProperty rdf:about="http://example.org/onto/prop/google_dialogflow_cx_flow_phone_number">
    <rdfs:label>phone_number</rdfs:label>
    <rdfs:comment>Transfer the call to a phone number in E.164 format.</rdfs:comment>
    <rdfs:domain rdf:resource="http://example.org/onto/class/google_dialogflow_cx_flow"/>
    <rdfs:range rdf:resource="http://www.w3.org/2001/XMLSchema#string"/>
  </owl:DatatypeProperty>
  <owl:DatatypeProperty rdf:about="http://example.org/onto/prop/google_dialogflow_cx_flow_allow_playback_interruption">
    <rdfs:label>allow_playback_interruption</rdfs:label>
    <rdfs:comment>Whether the playback of this message can be interrupted by the end user's speech and the client can then starts the next Dialogflow request.</rdfs:comment>
    <rdfs:domain rdf:resource="http://example.org/onto/class/google_dialogflow_cx_flow"/>
    <rdfs:range rdf:resource="http://www.w3.org/2001/XMLSchema#string"/>
  </owl:DatatypeProperty>
  <owl:DatatypeProperty rdf:about="http://example.org/onto/prop/google_dialogflow_cx_flow_text">
    <rdfs:label>text</rdfs:label>
    <rdfs:comment>A collection of text response variants. If multiple variants are defined, only one text response variant is returned at runtime.
required: true</rdfs:comment>
    <rdfs:domain rdf:resource="http://example.org/onto/class/google_dialogflow_cx_flow"/>
    <rdfs:range rdf:resource="http://www.w3.org/2001/XMLSchema#string"/>
  </owl:DatatypeProperty>
  <owl:DatatypeProperty rdf:about="http://example.org/onto/prop/google_dialogflow_cx_flow_parameter">
    <rdfs:label>parameter</rdfs:label>
    <rdfs:comment>Display name of the parameter.</rdfs:comment>
    <rdfs:domain rdf:resource="http://example.org/onto/class/google_dialogflow_cx_flow"/>
    <rdfs:range rdf:resource="http://www.w3.org/2001/XMLSchema#string"/>
  </owl:DatatypeProperty>
  <owl:DatatypeProperty rdf:about="http://example.org/onto/prop/google_dialogflow_cx_flow_value">
    <rdfs:label>value</rdfs:label>
    <rdfs:comment>The new JSON-encoded value of the parameter. A null value clears the parameter.</rdfs:comment>
    <rdfs:domain rdf:resource="http://example.org/onto/class/google_dialogflow_cx_flow"/>
    <rdfs:range rdf:resource="http://www.w3.org/2001/XMLSchema#string"/>
  </owl:DatatypeProperty>
  <owl:DatatypeProperty rdf:about="http://example.org/onto/prop/google_dialogflow_cx_flow_classification_threshold">
    <rdfs:label>classification_threshold</rdfs:label>
    <rdfs:comment>To filter out false positive results and still get variety in matched natural language inputs for your agent, you can tune the machine learning classification threshold.
If the returned score value is less than the threshold value, then a no-match event will be triggered. The score values range from 0.0 (completely uncertain) to 1.0 (completely certain). If set to 0.0, the default of 0.3 is used.</rdfs:comment>
    <rdfs:domain rdf:resource="http://example.org/onto/class/google_dialogflow_cx_flow"/>
    <rdfs:range rdf:resource="http://www.w3.org/2001/XMLSchema#string"/>
  </owl:DatatypeProperty>
  <owl:DatatypeProperty rdf:about="http://example.org/onto/prop/google_dialogflow_cx_flow_model_training_mode">
    <rdfs:label>model_training_mode</rdfs:label>
    <rdfs:comment>Indicates NLU model training mode.
* MODEL_TRAINING_MODE_AUTOMATIC: NLU model training is automatically triggered when a flow gets modified. User can also manually trigger model training in this mode.
* MODEL_TRAINING_MODE_MANUAL: User needs to manually trigger NLU model training. Best for large flows whose models take long time to train. Possible values: ["MODEL_TRAINING_MODE_AUTOMATIC", "MODEL_TRAINING_MODE_MANUAL"]</rdfs:comment>
    <rdfs:domain rdf:resource="http://example.org/onto/class/google_dialogflow_cx_flow"/>
    <rdfs:range rdf:resource="http://www.w3.org/2001/XMLSchema#string"/>
  </owl:DatatypeProperty>
  <owl:DatatypeProperty rdf:about="http://example.org/onto/prop/google_dialogflow_cx_flow_model_type">
    <rdfs:label>model_type</rdfs:label>
    <rdfs:comment>Indicates the type of NLU model.
* MODEL_TYPE_STANDARD: Use standard NLU model.
* MODEL_TYPE_ADVANCED: Use advanced NLU model. Possible values: ["MODEL_TYPE_STANDARD", "MODEL_TYPE_ADVANCED"]</rdfs:comment>
    <rdfs:domain rdf:resource="http://example.org/onto/class/google_dialogflow_cx_flow"/>
    <rdfs:range rdf:resource="http://www.w3.org/2001/XMLSchema#string"/>
  </owl:DatatypeProperty>
  <owl:DatatypeProperty rdf:about="http://example.org/onto/prop/google_dialogflow_cx_flow_create">
    <rdfs:label>create</rdfs:label>
    <rdfs:domain rdf:resource="http://example.org/onto/class/google_dialogflow_cx_flow"/>
    <rdfs:range rdf:resource="http://www.w3.org/2001/XMLSchema#string"/>
  </owl:DatatypeProperty>
  <owl:DatatypeProperty rdf:about="http://example.org/onto/prop/google_dialogflow_cx_flow_delete">
    <rdfs:label>delete</rdfs:label>
    <rdfs:domain rdf:resource="http://example.org/onto/class/google_dialogflow_cx_flow"/>
    <rdfs:range rdf:resource="http://www.w3.org/2001/XMLSchema#string"/>
  </owl:DatatypeProperty>
  <owl:DatatypeProperty rdf:about="http://example.org/onto/prop/google_dialogflow_cx_flow_update">
    <rdfs:label>update</rdfs:label>
    <rdfs:domain rdf:resource="http://example.org/onto/class/google_dialogflow_cx_flow"/>
    <rdfs:range rdf:resource="http://www.w3.org/2001/XMLSchema#string"/>
  </owl:DatatypeProperty>
  <owl:DatatypeProperty rdf:about="http://example.org/onto/prop/google_dialogflow_cx_flow_condition">
    <rdfs:label>condition</rdfs:label>
    <rdfs:comment>The condition to evaluate against form parameters or session parameters.
At least one of intent or condition must be specified. When both intent and condition are specified, the transition can only happen when both are fulfilled.</rdfs:comment>
    <rdfs:domain rdf:resource="http://example.org/onto/class/google_dialogflow_cx_flow"/>
    <rdfs:range rdf:resource="http://www.w3.org/2001/XMLSchema#string"/>
  </owl:DatatypeProperty>
  <owl:DatatypeProperty rdf:about="http://example.org/onto/prop/google_dialogflow_cx_flow_intent">
    <rdfs:label>intent</rdfs:label>
    <rdfs:comment>The unique identifier of an Intent.
Format: projects/<Project ID>/locations/<Location ID>/agents/<Agent ID>/intents/<Intent ID>. Indicates that the transition can only happen when the given intent is matched. At least one of intent or condition must be specified. When both intent and condition are specified, the transition can only happen when both are fulfilled.</rdfs:comment>
    <rdfs:domain rdf:resource="http://example.org/onto/class/google_dialogflow_cx_flow"/>
    <rdfs:range rdf:resource="http://www.w3.org/2001/XMLSchema#string"/>
  </owl:DatatypeProperty>
  <owl:DatatypeProperty rdf:about="http://example.org/onto/prop/google_dialogflow_cx_flow_name">
    <rdfs:label>name</rdfs:label>
    <rdfs:comment>The unique identifier of this transition route.</rdfs:comment>
    <rdfs:domain rdf:resource="http://example.org/onto/class/google_dialogflow_cx_flow"/>
    <rdfs:range rdf:resource="http://www.w3.org/2001/XMLSchema#string"/>
  </owl:DatatypeProperty>
  <owl:DatatypeProperty rdf:about="http://example.org/onto/prop/google_dialogflow_cx_flow_target_flow">
    <rdfs:label>target_flow</rdfs:label>
    <rdfs:comment>The target flow to transition to.
Format: projects/<Project ID>/locations/<Location ID>/agents/<Agent ID>/flows/<Flow ID>.</rdfs:comment>
    <rdfs:domain rdf:resource="http://example.org/onto/class/google_dialogflow_cx_flow"/>
    <rdfs:range rdf:resource="http://www.w3.org/2001/XMLSchema#string"/>
  </owl:DatatypeProperty>
  <owl:DatatypeProperty rdf:about="http://example.org/onto/prop/google_dialogflow_cx_flow_target_page">
    <rdfs:label>target_page</rdfs:label>
    <rdfs:comment>The target page to transition to.
Format: projects/<Project ID>/locations/<Location ID>/agents/<Agent ID>/flows/<Flow ID>/pages/<Page ID>.</rdfs:comment>
    <rdfs:domain rdf:resource="http://example.org/onto/class/google_dialogflow_cx_flow"/>
    <rdfs:range rdf:resource="http://www.w3.org/2001/XMLSchema#string"/>
  </owl:DatatypeProperty>
  <owl:DatatypeProperty rdf:about="http://example.org/onto/prop/google_dialogflow_cx_flow_return_partial_responses">
    <rdfs:label>return_partial_responses</rdfs:label>
    <rdfs:comment>Whether Dialogflow should return currently queued fulfillment response messages in streaming APIs. If a webhook is specified, it happens before Dialogflow invokes webhook. Warning: 1) This flag only affects streaming API. Responses are still queued and returned once in non-streaming API. 2) The flag can be enabled in any fulfillment but only the first 3 partial responses will be returned. You may only want to apply it to fulfillments that have slow webhooks.</rdfs:comment>
    <rdfs:domain rdf:resource="http://example.org/onto/class/google_dialogflow_cx_flow"/>
    <rdfs:range rdf:resource="http://www.w3.org/2001/XMLSchema#string"/>
  </owl:DatatypeProperty>
  <owl:DatatypeProperty rdf:about="http://example.org/onto/prop/google_dialogflow_cx_flow_tag">
    <rdfs:label>tag</rdfs:label>
    <rdfs:comment>The tag used by the webhook to identify which fulfillment is being called. This field is required if webhook is specified.</rdfs:comment>
    <rdfs:domain rdf:resource="http://example.org/onto/class/google_dialogflow_cx_flow"/>
    <rdfs:range rdf:resource="http://www.w3.org/2001/XMLSchema#string"/>
  </owl:DatatypeProperty>
  <owl:DatatypeProperty rdf:about="http://example.org/onto/prop/google_dialogflow_cx_flow_webhook">
    <rdfs:label>webhook</rdfs:label>
    <rdfs:comment>The webhook to call. Format: projects/<Project ID>/locations/<Location ID>/agents/<Agent ID>/webhooks/<Webhook ID>.</rdfs:comment>
    <rdfs:domain rdf:resource="http://example.org/onto/class/google_dialogflow_cx_flow"/>
    <rdfs:range rdf:resource="http://www.w3.org/2001/XMLSchema#string"/>
  </owl:DatatypeProperty>
  <owl:DatatypeProperty rdf:about="http://example.org/onto/prop/google_dialogflow_cx_flow_cases">
    <rdfs:label>cases</rdfs:label>
    <rdfs:comment>A JSON encoded list of cascading if-else conditions. Cases are mutually exclusive. The first one with a matching condition is selected, all the rest ignored.
See [Case](https://cloud.google.com/dialogflow/cx/docs/reference/rest/v3/Fulfillment#case) for the schema.</rdfs:comment>
    <rdfs:domain rdf:resource="http://example.org/onto/class/google_dialogflow_cx_flow"/>
    <rdfs:range rdf:resource="http://www.w3.org/2001/XMLSchema#string"/>
  </owl:DatatypeProperty>
  <owl:DatatypeProperty rdf:about="http://example.org/onto/prop/google_dialogflow_cx_flow_channel">
    <rdfs:label>channel</rdfs:label>
    <rdfs:comment>The channel which the response is associated with. Clients can specify the channel via QueryParameters.channel, and only associated channel response will be returned.</rdfs:comment>
    <rdfs:domain rdf:resource="http://example.org/onto/class/google_dialogflow_cx_flow"/>
    <rdfs:range rdf:resource="http://www.w3.org/2001/XMLSchema#string"/>
  </owl:DatatypeProperty>
  <owl:DatatypeProperty rdf:about="http://example.org/onto/prop/google_dialogflow_cx_flow_payload">
    <rdfs:label>payload</rdfs:label>
    <rdfs:comment>A custom, platform-specific payload.</rdfs:comment>
    <rdfs:domain rdf:resource="http://example.org/onto/class/google_dialogflow_cx_flow"/>
    <rdfs:range rdf:resource="http://www.w3.org/2001/XMLSchema#string"/>
  </owl:DatatypeProperty>
  <owl:DatatypeProperty rdf:about="http://example.org/onto/prop/google_dialogflow_cx_flow_metadata">
    <rdfs:label>metadata</rdfs:label>
    <rdfs:comment>Custom metadata. Dialogflow doesn't impose any structure on this.</rdfs:comment>
    <rdfs:domain rdf:resource="http://example.org/onto/class/google_dialogflow_cx_flow"/>
    <rdfs:range rdf:resource="http://www.w3.org/2001/XMLSchema#string"/>
  </owl:DatatypeProperty>
  <owl:DatatypeProperty rdf:about="http://example.org/onto/prop/google_dialogflow_cx_flow_metadata">
    <rdfs:label>metadata</rdfs:label>
    <rdfs:comment>Custom metadata. Dialogflow doesn't impose any structure on this.</rdfs:comment>
    <rdfs:domain rdf:resource="http://example.org/onto/class/google_dialogflow_cx_flow"/>
    <rdfs:range rdf:resource="http://www.w3.org/2001/XMLSchema#string"/>
  </owl:DatatypeProperty>
  <owl:DatatypeProperty rdf:about="http://example.org/onto/prop/google_dialogflow_cx_flow_allow_playback_interruption">
    <rdfs:label>allow_playback_interruption</rdfs:label>
    <rdfs:comment>Whether the playback of this message can be interrupted by the end user's speech and the client can then starts the next Dialogflow request.</rdfs:comment>
    <rdfs:domain rdf:resource="http://example.org/onto/class/google_dialogflow_cx_flow"/>
    <rdfs:range rdf:resource="http://www.w3.org/2001/XMLSchema#string"/>
  </owl:DatatypeProperty>
  <owl:DatatypeProperty rdf:about="http://example.org/onto/prop/google_dialogflow_cx_flow_ssml">
    <rdfs:label>ssml</rdfs:label>
    <rdfs:comment>The SSML text to be synthesized. For more information, see SSML.</rdfs:comment>
    <rdfs:domain rdf:resource="http://example.org/onto/class/google_dialogflow_cx_flow"/>
    <rdfs:range rdf:resource="http://www.w3.org/2001/XMLSchema#string"/>
  </owl:DatatypeProperty>
  <owl:DatatypeProperty rdf:about="http://example.org/onto/prop/google_dialogflow_cx_flow_text">
    <rdfs:label>text</rdfs:label>
    <rdfs:comment>The raw text to be synthesized.</rdfs:comment>
    <rdfs:domain rdf:resource="http://example.org/onto/class/google_dialogflow_cx_flow"/>
    <rdfs:range rdf:resource="http://www.w3.org/2001/XMLSchema#string"/>
  </owl:DatatypeProperty>
  <owl:DatatypeProperty rdf:about="http://example.org/onto/prop/google_dialogflow_cx_flow_allow_playback_interruption">
    <rdfs:label>allow_playback_interruption</rdfs:label>
    <rdfs:comment>Whether the playback of this message can be interrupted by the end user's speech and the client can then starts the next Dialogflow request.</rdfs:comment>
    <rdfs:domain rdf:resource="http://example.org/onto/class/google_dialogflow_cx_flow"/>
    <rdfs:range rdf:resource="http://www.w3.org/2001/XMLSchema#string"/>
  </owl:DatatypeProperty>
  <owl:DatatypeProperty rdf:about="http://example.org/onto/prop/google_dialogflow_cx_flow_audio_uri">
    <rdfs:label>audio_uri</rdfs:label>
    <rdfs:comment>URI of the audio clip. Dialogflow does not impose any validation on this value. It is specific to the client that reads it.</rdfs:comment>
    <rdfs:domain rdf:resource="http://example.org/onto/class/google_dialogflow_cx_flow"/>
    <rdfs:range rdf:resource="http://www.w3.org/2001/XMLSchema#string"/>
  </owl:DatatypeProperty>
  <owl:DatatypeProperty rdf:about="http://example.org/onto/prop/google_dialogflow_cx_flow_phone_number">
    <rdfs:label>phone_number</rdfs:label>
    <rdfs:comment>Transfer the call to a phone number in E.164 format.</rdfs:comment>
    <rdfs:domain rdf:resource="http://example.org/onto/class/google_dialogflow_cx_flow"/>
    <rdfs:range rdf:resource="http://www.w3.org/2001/XMLSchema#string"/>
  </owl:DatatypeProperty>
  <owl:DatatypeProperty rdf:about="http://example.org/onto/prop/google_dialogflow_cx_flow_allow_playback_interruption">
    <rdfs:label>allow_playback_interruption</rdfs:label>
    <rdfs:comment>Whether the playback of this message can be interrupted by the end user's speech and the client can then starts the next Dialogflow request.</rdfs:comment>
    <rdfs:domain rdf:resource="http://example.org/onto/class/google_dialogflow_cx_flow"/>
    <rdfs:range rdf:resource="http://www.w3.org/2001/XMLSchema#string"/>
  </owl:DatatypeProperty>
  <owl:DatatypeProperty rdf:about="http://example.org/onto/prop/google_dialogflow_cx_flow_text">
    <rdfs:label>text</rdfs:label>
    <rdfs:comment>A collection of text responses.</rdfs:comment>
    <rdfs:domain rdf:resource="http://example.org/onto/class/google_dialogflow_cx_flow"/>
    <rdfs:range rdf:resource="http://www.w3.org/2001/XMLSchema#string"/>
  </owl:DatatypeProperty>
  <owl:DatatypeProperty rdf:about="http://example.org/onto/prop/google_dialogflow_cx_flow_parameter">
    <rdfs:label>parameter</rdfs:label>
    <rdfs:comment>Display name of the parameter.</rdfs:comment>
    <rdfs:domain rdf:resource="http://example.org/onto/class/google_dialogflow_cx_flow"/>
    <rdfs:range rdf:resource="http://www.w3.org/2001/XMLSchema#string"/>
  </owl:DatatypeProperty>
  <owl:DatatypeProperty rdf:about="http://example.org/onto/prop/google_dialogflow_cx_flow_value">
    <rdfs:label>value</rdfs:label>
    <rdfs:comment>The new JSON-encoded value of the parameter. A null value clears the parameter.</rdfs:comment>
    <rdfs:domain rdf:resource="http://example.org/onto/class/google_dialogflow_cx_flow"/>
    <rdfs:range rdf:resource="http://www.w3.org/2001/XMLSchema#string"/>
  </owl:DatatypeProperty>
</rdf:RDF>
