<?xml version="1.0" encoding="UTF-8"?>
<rdf:RDF
  xmlns:rdf="http://www.w3.org/1999/02/22-rdf-syntax-ns#"
  xmlns:rdfs="http://www.w3.org/2000/01/rdf-schema#"
  xmlns:owl="http://www.w3.org/2002/07/owl#"
  xmlns:xsd="http://www.w3.org/2001/XMLSchema#"
  xml:base="http://example.org/onto/">
  <owl:Class rdf:about="http://example.org/onto/class/google_public_ca_external_account_key">
    <rdfs:label>google_public_ca_external_account_key</rdfs:label>
    <rdfs:comment>#
#     ***     AUTO GENERATED CODE    ***    Type: MMv1     ***
#
# ----------------------------------------------------------------------------
#
#     This code is generated by Magic Modules using the following:
#
#     Configuration: https:#github.com/GoogleCloudPlatform/magic-modules/tree/main/mmv1/products/publicca/ExternalAccountKey.yaml
#     Template:      https:#github.com/GoogleCloudPlatform/magic-modules/tree/main/mmv1/templates/terraform/resource.html.markdown.tmpl
#
#     DO NOT EDIT this file directly. Any changes made to this file will be
#     overwritten during the next generation cycle.
#
# ----------------------------------------------------------------------------
subcategory: "Public CA"
description: |-
  A representation of an ExternalAccountKey used for external account binding within ACME.
---</rdfs:comment>
  </owl:Class>
  <owl:DatatypeProperty rdf:about="http://example.org/onto/prop/google_public_ca_external_account_key_b64_mac_key">
    <rdfs:label>b64_mac_key</rdfs:label>
    <rdfs:comment>Base64-URL-encoded HS256 key. It is generated by the PublicCertificateAuthorityService
when the ExternalAccountKey is created.</rdfs:comment>
    <rdfs:domain rdf:resource="http://example.org/onto/class/google_public_ca_external_account_key"/>
    <rdfs:range rdf:resource="http://www.w3.org/2001/XMLSchema#string"/>
  </owl:DatatypeProperty>
  <owl:DatatypeProperty rdf:about="http://example.org/onto/prop/google_public_ca_external_account_key_b64url_mac_key">
    <rdfs:label>b64url_mac_key</rdfs:label>
    <rdfs:comment>Base64-URL-encoded HS256 key. It is generated by the PublicCertificateAuthorityService
when the ExternalAccountKey is created.'</rdfs:comment>
    <rdfs:domain rdf:resource="http://example.org/onto/class/google_public_ca_external_account_key"/>
    <rdfs:range rdf:resource="http://www.w3.org/2001/XMLSchema#string"/>
  </owl:DatatypeProperty>
  <owl:DatatypeProperty rdf:about="http://example.org/onto/prop/google_public_ca_external_account_key_id">
    <rdfs:label>id</rdfs:label>
    <rdfs:domain rdf:resource="http://example.org/onto/class/google_public_ca_external_account_key"/>
    <rdfs:range rdf:resource="http://www.w3.org/2001/XMLSchema#string"/>
  </owl:DatatypeProperty>
  <owl:DatatypeProperty rdf:about="http://example.org/onto/prop/google_public_ca_external_account_key_key_id">
    <rdfs:label>key_id</rdfs:label>
    <rdfs:comment>It is generated by the PublicCertificateAuthorityService when the ExternalAccountKey is created.</rdfs:comment>
    <rdfs:domain rdf:resource="http://example.org/onto/class/google_public_ca_external_account_key"/>
    <rdfs:range rdf:resource="http://www.w3.org/2001/XMLSchema#string"/>
  </owl:DatatypeProperty>
  <owl:DatatypeProperty rdf:about="http://example.org/onto/prop/google_public_ca_external_account_key_location">
    <rdfs:label>location</rdfs:label>
    <rdfs:comment>Location for the externalAccountKey. Currently only 'global' is supported.</rdfs:comment>
    <rdfs:domain rdf:resource="http://example.org/onto/class/google_public_ca_external_account_key"/>
    <rdfs:range rdf:resource="http://www.w3.org/2001/XMLSchema#string"/>
  </owl:DatatypeProperty>
  <owl:DatatypeProperty rdf:about="http://example.org/onto/prop/google_public_ca_external_account_key_name">
    <rdfs:label>name</rdfs:label>
    <rdfs:comment>Resource name. projects/{project}/locations/{location}/externalAccountKeys/{keyId}.</rdfs:comment>
    <rdfs:domain rdf:resource="http://example.org/onto/class/google_public_ca_external_account_key"/>
    <rdfs:range rdf:resource="http://www.w3.org/2001/XMLSchema#string"/>
  </owl:DatatypeProperty>
  <owl:DatatypeProperty rdf:about="http://example.org/onto/prop/google_public_ca_external_account_key_project">
    <rdfs:label>project</rdfs:label>
    <rdfs:domain rdf:resource="http://example.org/onto/class/google_public_ca_external_account_key"/>
    <rdfs:range rdf:resource="http://www.w3.org/2001/XMLSchema#string"/>
  </owl:DatatypeProperty>
  <owl:DatatypeProperty rdf:about="http://example.org/onto/prop/google_public_ca_external_account_key_create">
    <rdfs:label>create</rdfs:label>
    <rdfs:domain rdf:resource="http://example.org/onto/class/google_public_ca_external_account_key"/>
    <rdfs:range rdf:resource="http://www.w3.org/2001/XMLSchema#string"/>
  </owl:DatatypeProperty>
  <owl:DatatypeProperty rdf:about="http://example.org/onto/prop/google_public_ca_external_account_key_delete">
    <rdfs:label>delete</rdfs:label>
    <rdfs:domain rdf:resource="http://example.org/onto/class/google_public_ca_external_account_key"/>
    <rdfs:range rdf:resource="http://www.w3.org/2001/XMLSchema#string"/>
  </owl:DatatypeProperty>
</rdf:RDF>
