<?xml version="1.0" encoding="UTF-8"?>
<rdf:RDF
  xmlns:rdf="http://www.w3.org/1999/02/22-rdf-syntax-ns#"
  xmlns:rdfs="http://www.w3.org/2000/01/rdf-schema#"
  xmlns:owl="http://www.w3.org/2002/07/owl#"
  xmlns:xsd="http://www.w3.org/2001/XMLSchema#"
  xml:base="http://example.org/onto/">
  <owl:Class rdf:about="http://example.org/onto/class/google_gkeonprem_bare_metal_admin_cluster">
    <rdfs:label>google_gkeonprem_bare_metal_admin_cluster</rdfs:label>
    <rdfs:comment>#
#     ***     AUTO GENERATED CODE    ***    Type: MMv1     ***
#
# ----------------------------------------------------------------------------
#
#     This code is generated by Magic Modules using the following:
#
#     Configuration: https:#github.com/GoogleCloudPlatform/magic-modules/tree/main/mmv1/products/gkeonprem/BareMetalAdminCluster.yaml
#     Template:      https:#github.com/GoogleCloudPlatform/magic-modules/tree/main/mmv1/templates/terraform/resource.html.markdown.tmpl
#
#     DO NOT EDIT this file directly. Any changes made to this file will be
#     overwritten during the next generation cycle.
#
# ----------------------------------------------------------------------------
subcategory: "Anthos On-Prem"
description: |-
  A Google Bare Metal Admin Cluster.
---</rdfs:comment>
  </owl:Class>
  <owl:DatatypeProperty rdf:about="http://example.org/onto/prop/google_gkeonprem_bare_metal_admin_cluster_annotations">
    <rdfs:label>annotations</rdfs:label>
    <rdfs:comment>Annotations on the Bare Metal Admin Cluster.
This field has the same restrictions as Kubernetes annotations.
The total size of all keys and values combined is limited to 256k.
Key can have 2 segments: prefix (optional) and name (required),
separated by a slash (/).
Prefix must be a DNS subdomain.
Name must be 63 characters or less, begin and end with alphanumerics,
with dashes (-), underscores (_), dots (.), and alphanumerics between.


**Note**: This field is non-authoritative, and will only manage the annotations present in your configuration.
Please refer to the field 'effective_annotations' for all of the annotations present on the resource.</rdfs:comment>
    <rdfs:domain rdf:resource="http://example.org/onto/class/google_gkeonprem_bare_metal_admin_cluster"/>
    <rdfs:range rdf:resource="http://www.w3.org/2001/XMLSchema#string"/>
  </owl:DatatypeProperty>
  <owl:DatatypeProperty rdf:about="http://example.org/onto/prop/google_gkeonprem_bare_metal_admin_cluster_bare_metal_version">
    <rdfs:label>bare_metal_version</rdfs:label>
    <rdfs:comment>A human readable description of this Bare Metal Admin Cluster.</rdfs:comment>
    <rdfs:domain rdf:resource="http://example.org/onto/class/google_gkeonprem_bare_metal_admin_cluster"/>
    <rdfs:range rdf:resource="http://www.w3.org/2001/XMLSchema#string"/>
  </owl:DatatypeProperty>
  <owl:DatatypeProperty rdf:about="http://example.org/onto/prop/google_gkeonprem_bare_metal_admin_cluster_create_time">
    <rdfs:label>create_time</rdfs:label>
    <rdfs:comment>The time the cluster was created, in RFC3339 text format.</rdfs:comment>
    <rdfs:domain rdf:resource="http://example.org/onto/class/google_gkeonprem_bare_metal_admin_cluster"/>
    <rdfs:range rdf:resource="http://www.w3.org/2001/XMLSchema#string"/>
  </owl:DatatypeProperty>
  <owl:DatatypeProperty rdf:about="http://example.org/onto/prop/google_gkeonprem_bare_metal_admin_cluster_delete_time">
    <rdfs:label>delete_time</rdfs:label>
    <rdfs:comment>The time the cluster was deleted, in RFC3339 text format.</rdfs:comment>
    <rdfs:domain rdf:resource="http://example.org/onto/class/google_gkeonprem_bare_metal_admin_cluster"/>
    <rdfs:range rdf:resource="http://www.w3.org/2001/XMLSchema#string"/>
  </owl:DatatypeProperty>
  <owl:DatatypeProperty rdf:about="http://example.org/onto/prop/google_gkeonprem_bare_metal_admin_cluster_description">
    <rdfs:label>description</rdfs:label>
    <rdfs:comment>A human readable description of this Bare Metal Admin Cluster.</rdfs:comment>
    <rdfs:domain rdf:resource="http://example.org/onto/class/google_gkeonprem_bare_metal_admin_cluster"/>
    <rdfs:range rdf:resource="http://www.w3.org/2001/XMLSchema#string"/>
  </owl:DatatypeProperty>
  <owl:DatatypeProperty rdf:about="http://example.org/onto/prop/google_gkeonprem_bare_metal_admin_cluster_effective_annotations">
    <rdfs:label>effective_annotations</rdfs:label>
    <rdfs:comment>All of annotations (key/value pairs) present on the resource in GCP, including the annotations configured through Terraform, other clients and services.</rdfs:comment>
    <rdfs:domain rdf:resource="http://example.org/onto/class/google_gkeonprem_bare_metal_admin_cluster"/>
    <rdfs:range rdf:resource="http://www.w3.org/2001/XMLSchema#string"/>
  </owl:DatatypeProperty>
  <owl:DatatypeProperty rdf:about="http://example.org/onto/prop/google_gkeonprem_bare_metal_admin_cluster_endpoint">
    <rdfs:label>endpoint</rdfs:label>
    <rdfs:comment>The IP address name of Bare Metal Admin Cluster's API server.</rdfs:comment>
    <rdfs:domain rdf:resource="http://example.org/onto/class/google_gkeonprem_bare_metal_admin_cluster"/>
    <rdfs:range rdf:resource="http://www.w3.org/2001/XMLSchema#string"/>
  </owl:DatatypeProperty>
  <owl:DatatypeProperty rdf:about="http://example.org/onto/prop/google_gkeonprem_bare_metal_admin_cluster_etag">
    <rdfs:label>etag</rdfs:label>
    <rdfs:comment>This checksum is computed by the server based on the value of other
fields, and may be sent on update and delete requests to ensure the
client has an up-to-date value before proceeding.
Allows clients to perform consistent read-modify-writes
through optimistic concurrency control.</rdfs:comment>
    <rdfs:domain rdf:resource="http://example.org/onto/class/google_gkeonprem_bare_metal_admin_cluster"/>
    <rdfs:range rdf:resource="http://www.w3.org/2001/XMLSchema#string"/>
  </owl:DatatypeProperty>
  <owl:DatatypeProperty rdf:about="http://example.org/onto/prop/google_gkeonprem_bare_metal_admin_cluster_fleet">
    <rdfs:label>fleet</rdfs:label>
    <rdfs:comment>Fleet related configuration.
Fleets are a Google Cloud concept for logically organizing clusters,
letting you use and manage multi-cluster capabilities and apply
consistent policies across your systems.
See [Anthos Fleets](https://cloud.google.com/anthos/multicluster-management/fleets) for
more details on Anthos multi-cluster capabilities using Fleets.</rdfs:comment>
    <rdfs:domain rdf:resource="http://example.org/onto/class/google_gkeonprem_bare_metal_admin_cluster"/>
    <rdfs:range rdf:resource="http://www.w3.org/2001/XMLSchema#string"/>
  </owl:DatatypeProperty>
  <owl:DatatypeProperty rdf:about="http://example.org/onto/prop/google_gkeonprem_bare_metal_admin_cluster_id">
    <rdfs:label>id</rdfs:label>
    <rdfs:domain rdf:resource="http://example.org/onto/class/google_gkeonprem_bare_metal_admin_cluster"/>
    <rdfs:range rdf:resource="http://www.w3.org/2001/XMLSchema#string"/>
  </owl:DatatypeProperty>
  <owl:DatatypeProperty rdf:about="http://example.org/onto/prop/google_gkeonprem_bare_metal_admin_cluster_local_name">
    <rdfs:label>local_name</rdfs:label>
    <rdfs:comment>The object name of the Bare Metal Admin Cluster custom resource on the
associated admin cluster. This field is used to support conflicting
names when enrolling existing clusters to the API. When used as a part of
cluster enrollment, this field will differ from the ID in the resource
name. For new clusters, this field will match the user provided cluster ID
and be visible in the last component of the resource name. It is not
modifiable.
All users should use this name to access their cluster using gkectl or
kubectl and should expect to see the local name when viewing admin
cluster controller logs.</rdfs:comment>
    <rdfs:domain rdf:resource="http://example.org/onto/class/google_gkeonprem_bare_metal_admin_cluster"/>
    <rdfs:range rdf:resource="http://www.w3.org/2001/XMLSchema#string"/>
  </owl:DatatypeProperty>
  <owl:DatatypeProperty rdf:about="http://example.org/onto/prop/google_gkeonprem_bare_metal_admin_cluster_location">
    <rdfs:label>location</rdfs:label>
    <rdfs:comment>The location of the resource.</rdfs:comment>
    <rdfs:domain rdf:resource="http://example.org/onto/class/google_gkeonprem_bare_metal_admin_cluster"/>
    <rdfs:range rdf:resource="http://www.w3.org/2001/XMLSchema#string"/>
  </owl:DatatypeProperty>
  <owl:DatatypeProperty rdf:about="http://example.org/onto/prop/google_gkeonprem_bare_metal_admin_cluster_name">
    <rdfs:label>name</rdfs:label>
    <rdfs:comment>The bare metal admin cluster name.</rdfs:comment>
    <rdfs:domain rdf:resource="http://example.org/onto/class/google_gkeonprem_bare_metal_admin_cluster"/>
    <rdfs:range rdf:resource="http://www.w3.org/2001/XMLSchema#string"/>
  </owl:DatatypeProperty>
  <owl:DatatypeProperty rdf:about="http://example.org/onto/prop/google_gkeonprem_bare_metal_admin_cluster_project">
    <rdfs:label>project</rdfs:label>
    <rdfs:domain rdf:resource="http://example.org/onto/class/google_gkeonprem_bare_metal_admin_cluster"/>
    <rdfs:range rdf:resource="http://www.w3.org/2001/XMLSchema#string"/>
  </owl:DatatypeProperty>
  <owl:DatatypeProperty rdf:about="http://example.org/onto/prop/google_gkeonprem_bare_metal_admin_cluster_reconciling">
    <rdfs:label>reconciling</rdfs:label>
    <rdfs:comment>If set, there are currently changes in flight to the Bare Metal Admin Cluster.</rdfs:comment>
    <rdfs:domain rdf:resource="http://example.org/onto/class/google_gkeonprem_bare_metal_admin_cluster"/>
    <rdfs:range rdf:resource="http://www.w3.org/2001/XMLSchema#string"/>
  </owl:DatatypeProperty>
  <owl:DatatypeProperty rdf:about="http://example.org/onto/prop/google_gkeonprem_bare_metal_admin_cluster_state">
    <rdfs:label>state</rdfs:label>
    <rdfs:comment>The current state of this cluster.</rdfs:comment>
    <rdfs:domain rdf:resource="http://example.org/onto/class/google_gkeonprem_bare_metal_admin_cluster"/>
    <rdfs:range rdf:resource="http://www.w3.org/2001/XMLSchema#string"/>
  </owl:DatatypeProperty>
  <owl:DatatypeProperty rdf:about="http://example.org/onto/prop/google_gkeonprem_bare_metal_admin_cluster_status">
    <rdfs:label>status</rdfs:label>
    <rdfs:comment>Specifies detailed cluster status.</rdfs:comment>
    <rdfs:domain rdf:resource="http://example.org/onto/class/google_gkeonprem_bare_metal_admin_cluster"/>
    <rdfs:range rdf:resource="http://www.w3.org/2001/XMLSchema#string"/>
  </owl:DatatypeProperty>
  <owl:DatatypeProperty rdf:about="http://example.org/onto/prop/google_gkeonprem_bare_metal_admin_cluster_uid">
    <rdfs:label>uid</rdfs:label>
    <rdfs:comment>The unique identifier of the Bare Metal Admin Cluster.</rdfs:comment>
    <rdfs:domain rdf:resource="http://example.org/onto/class/google_gkeonprem_bare_metal_admin_cluster"/>
    <rdfs:range rdf:resource="http://www.w3.org/2001/XMLSchema#string"/>
  </owl:DatatypeProperty>
  <owl:DatatypeProperty rdf:about="http://example.org/onto/prop/google_gkeonprem_bare_metal_admin_cluster_update_time">
    <rdfs:label>update_time</rdfs:label>
    <rdfs:comment>The time the cluster was last updated, in RFC3339 text format.</rdfs:comment>
    <rdfs:domain rdf:resource="http://example.org/onto/class/google_gkeonprem_bare_metal_admin_cluster"/>
    <rdfs:range rdf:resource="http://www.w3.org/2001/XMLSchema#string"/>
  </owl:DatatypeProperty>
  <owl:DatatypeProperty rdf:about="http://example.org/onto/prop/google_gkeonprem_bare_metal_admin_cluster_validation_check">
    <rdfs:label>validation_check</rdfs:label>
    <rdfs:comment>Specifies the security related settings for the Bare Metal Admin Cluster.</rdfs:comment>
    <rdfs:domain rdf:resource="http://example.org/onto/class/google_gkeonprem_bare_metal_admin_cluster"/>
    <rdfs:range rdf:resource="http://www.w3.org/2001/XMLSchema#string"/>
  </owl:DatatypeProperty>
  <owl:DatatypeProperty rdf:about="http://example.org/onto/prop/google_gkeonprem_bare_metal_admin_cluster_enable_application_logs">
    <rdfs:label>enable_application_logs</rdfs:label>
    <rdfs:comment>Whether collection of application logs/metrics should be enabled (in addition to system logs/metrics).</rdfs:comment>
    <rdfs:domain rdf:resource="http://example.org/onto/class/google_gkeonprem_bare_metal_admin_cluster"/>
    <rdfs:range rdf:resource="http://www.w3.org/2001/XMLSchema#string"/>
  </owl:DatatypeProperty>
  <owl:DatatypeProperty rdf:about="http://example.org/onto/prop/google_gkeonprem_bare_metal_admin_cluster_argument">
    <rdfs:label>argument</rdfs:label>
    <rdfs:comment>The argument name as it appears on the API Server command line please make sure to remove the leading dashes.</rdfs:comment>
    <rdfs:domain rdf:resource="http://example.org/onto/class/google_gkeonprem_bare_metal_admin_cluster"/>
    <rdfs:range rdf:resource="http://www.w3.org/2001/XMLSchema#string"/>
  </owl:DatatypeProperty>
  <owl:DatatypeProperty rdf:about="http://example.org/onto/prop/google_gkeonprem_bare_metal_admin_cluster_value">
    <rdfs:label>value</rdfs:label>
    <rdfs:comment>The value of the arg as it will be passed to the API Server command line.</rdfs:comment>
    <rdfs:domain rdf:resource="http://example.org/onto/class/google_gkeonprem_bare_metal_admin_cluster"/>
    <rdfs:range rdf:resource="http://www.w3.org/2001/XMLSchema#string"/>
  </owl:DatatypeProperty>
  <owl:DatatypeProperty rdf:about="http://example.org/onto/prop/google_gkeonprem_bare_metal_admin_cluster_labels">
    <rdfs:label>labels</rdfs:label>
    <rdfs:comment>The map of Kubernetes labels (key/value pairs) to be applied to
each node. These will added in addition to any default label(s)
that Kubernetes may apply to the node. In case of conflict in
label keys, the applied set may differ depending on the Kubernetes
version -- it's best to assume the behavior is undefined and
conflicts should be avoided. For more information, including usage
and the valid values, see:
  - http://kubernetes.io/v1.1/docs/user-guide/labels.html
An object containing a list of "key": value pairs.
For example: { "name": "wrench", "mass": "1.3kg", "count": "3" }.</rdfs:comment>
    <rdfs:domain rdf:resource="http://example.org/onto/class/google_gkeonprem_bare_metal_admin_cluster"/>
    <rdfs:range rdf:resource="http://www.w3.org/2001/XMLSchema#string"/>
  </owl:DatatypeProperty>
  <owl:DatatypeProperty rdf:about="http://example.org/onto/prop/google_gkeonprem_bare_metal_admin_cluster_operating_system">
    <rdfs:label>operating_system</rdfs:label>
    <rdfs:comment>Specifies the nodes operating system (default: LINUX).</rdfs:comment>
    <rdfs:domain rdf:resource="http://example.org/onto/class/google_gkeonprem_bare_metal_admin_cluster"/>
    <rdfs:range rdf:resource="http://www.w3.org/2001/XMLSchema#string"/>
  </owl:DatatypeProperty>
  <owl:DatatypeProperty rdf:about="http://example.org/onto/prop/google_gkeonprem_bare_metal_admin_cluster_labels">
    <rdfs:label>labels</rdfs:label>
    <rdfs:comment>The map of Kubernetes labels (key/value pairs) to be applied to
each node. These will added in addition to any default label(s)
that Kubernetes may apply to the node. In case of conflict in
label keys, the applied set may differ depending on the Kubernetes
version -- it's best to assume the behavior is undefined and
conflicts should be avoided. For more information, including usage
and the valid values, see:
  - http://kubernetes.io/v1.1/docs/user-guide/labels.html
An object containing a list of "key": value pairs.
For example: { "name": "wrench", "mass": "1.3kg", "count": "3" }.</rdfs:comment>
    <rdfs:domain rdf:resource="http://example.org/onto/class/google_gkeonprem_bare_metal_admin_cluster"/>
    <rdfs:range rdf:resource="http://www.w3.org/2001/XMLSchema#string"/>
  </owl:DatatypeProperty>
  <owl:DatatypeProperty rdf:about="http://example.org/onto/prop/google_gkeonprem_bare_metal_admin_cluster_node_ip">
    <rdfs:label>node_ip</rdfs:label>
    <rdfs:comment>The default IPv4 address for SSH access and Kubernetes node.
Example: 192.168.0.1</rdfs:comment>
    <rdfs:domain rdf:resource="http://example.org/onto/class/google_gkeonprem_bare_metal_admin_cluster"/>
    <rdfs:range rdf:resource="http://www.w3.org/2001/XMLSchema#string"/>
  </owl:DatatypeProperty>
  <owl:DatatypeProperty rdf:about="http://example.org/onto/prop/google_gkeonprem_bare_metal_admin_cluster_effect">
    <rdfs:label>effect</rdfs:label>
    <rdfs:comment>Specifies the nodes operating system (default: LINUX). Possible values: ["EFFECT_UNSPECIFIED", "PREFER_NO_SCHEDULE", "NO_EXECUTE"]</rdfs:comment>
    <rdfs:domain rdf:resource="http://example.org/onto/class/google_gkeonprem_bare_metal_admin_cluster"/>
    <rdfs:range rdf:resource="http://www.w3.org/2001/XMLSchema#string"/>
  </owl:DatatypeProperty>
  <owl:DatatypeProperty rdf:about="http://example.org/onto/prop/google_gkeonprem_bare_metal_admin_cluster_key">
    <rdfs:label>key</rdfs:label>
    <rdfs:comment>Key associated with the effect.</rdfs:comment>
    <rdfs:domain rdf:resource="http://example.org/onto/class/google_gkeonprem_bare_metal_admin_cluster"/>
    <rdfs:range rdf:resource="http://www.w3.org/2001/XMLSchema#string"/>
  </owl:DatatypeProperty>
  <owl:DatatypeProperty rdf:about="http://example.org/onto/prop/google_gkeonprem_bare_metal_admin_cluster_value">
    <rdfs:label>value</rdfs:label>
    <rdfs:comment>Value associated with the effect.</rdfs:comment>
    <rdfs:domain rdf:resource="http://example.org/onto/class/google_gkeonprem_bare_metal_admin_cluster"/>
    <rdfs:range rdf:resource="http://www.w3.org/2001/XMLSchema#string"/>
  </owl:DatatypeProperty>
  <owl:DatatypeProperty rdf:about="http://example.org/onto/prop/google_gkeonprem_bare_metal_admin_cluster_enabled">
    <rdfs:label>enabled</rdfs:label>
    <rdfs:comment>Whether manual load balancing is enabled.</rdfs:comment>
    <rdfs:domain rdf:resource="http://example.org/onto/class/google_gkeonprem_bare_metal_admin_cluster"/>
    <rdfs:range rdf:resource="http://www.w3.org/2001/XMLSchema#string"/>
  </owl:DatatypeProperty>
  <owl:DatatypeProperty rdf:about="http://example.org/onto/prop/google_gkeonprem_bare_metal_admin_cluster_control_plane_load_balancer_port">
    <rdfs:label>control_plane_load_balancer_port</rdfs:label>
    <rdfs:comment>The port that control plane hosted load balancers will listen on.</rdfs:comment>
    <rdfs:domain rdf:resource="http://example.org/onto/class/google_gkeonprem_bare_metal_admin_cluster"/>
    <rdfs:range rdf:resource="http://www.w3.org/2001/XMLSchema#string"/>
  </owl:DatatypeProperty>
  <owl:DatatypeProperty rdf:about="http://example.org/onto/prop/google_gkeonprem_bare_metal_admin_cluster_control_plane_vip">
    <rdfs:label>control_plane_vip</rdfs:label>
    <rdfs:comment>The VIP which you previously set aside for the Kubernetes API of this Bare Metal Admin Cluster.</rdfs:comment>
    <rdfs:domain rdf:resource="http://example.org/onto/class/google_gkeonprem_bare_metal_admin_cluster"/>
    <rdfs:range rdf:resource="http://www.w3.org/2001/XMLSchema#string"/>
  </owl:DatatypeProperty>
  <owl:DatatypeProperty rdf:about="http://example.org/onto/prop/google_gkeonprem_bare_metal_admin_cluster_maintenance_address_cidr_blocks">
    <rdfs:label>maintenance_address_cidr_blocks</rdfs:label>
    <rdfs:comment>All IPv4 address from these ranges will be placed into maintenance mode.
Nodes in maintenance mode will be cordoned and drained. When both of these
are true, the "baremetal.cluster.gke.io/maintenance" annotation will be set
on the node resource.</rdfs:comment>
    <rdfs:domain rdf:resource="http://example.org/onto/class/google_gkeonprem_bare_metal_admin_cluster"/>
    <rdfs:range rdf:resource="http://www.w3.org/2001/XMLSchema#string"/>
  </owl:DatatypeProperty>
  <owl:DatatypeProperty rdf:about="http://example.org/onto/prop/google_gkeonprem_bare_metal_admin_cluster_pod_address_cidr_blocks">
    <rdfs:label>pod_address_cidr_blocks</rdfs:label>
    <rdfs:comment>All pods in the cluster are assigned an RFC1918 IPv4 address from these ranges. This field cannot be changed after creation.</rdfs:comment>
    <rdfs:domain rdf:resource="http://example.org/onto/class/google_gkeonprem_bare_metal_admin_cluster"/>
    <rdfs:range rdf:resource="http://www.w3.org/2001/XMLSchema#string"/>
  </owl:DatatypeProperty>
  <owl:DatatypeProperty rdf:about="http://example.org/onto/prop/google_gkeonprem_bare_metal_admin_cluster_service_address_cidr_blocks">
    <rdfs:label>service_address_cidr_blocks</rdfs:label>
    <rdfs:comment>All services in the cluster are assigned an RFC1918 IPv4 address from these ranges. This field cannot be changed after creation.</rdfs:comment>
    <rdfs:domain rdf:resource="http://example.org/onto/class/google_gkeonprem_bare_metal_admin_cluster"/>
    <rdfs:range rdf:resource="http://www.w3.org/2001/XMLSchema#string"/>
  </owl:DatatypeProperty>
  <owl:DatatypeProperty rdf:about="http://example.org/onto/prop/google_gkeonprem_bare_metal_admin_cluster_login_user">
    <rdfs:label>login_user</rdfs:label>
    <rdfs:comment>LoginUser is the user name used to access node machines.
It defaults to "root" if not set.</rdfs:comment>
    <rdfs:domain rdf:resource="http://example.org/onto/class/google_gkeonprem_bare_metal_admin_cluster"/>
    <rdfs:range rdf:resource="http://www.w3.org/2001/XMLSchema#string"/>
  </owl:DatatypeProperty>
  <owl:DatatypeProperty rdf:about="http://example.org/onto/prop/google_gkeonprem_bare_metal_admin_cluster_max_pods_per_node">
    <rdfs:label>max_pods_per_node</rdfs:label>
    <rdfs:comment>The maximum number of pods a node can run. The size of the CIDR range
assigned to the node will be derived from this parameter.</rdfs:comment>
    <rdfs:domain rdf:resource="http://example.org/onto/class/google_gkeonprem_bare_metal_admin_cluster"/>
    <rdfs:range rdf:resource="http://www.w3.org/2001/XMLSchema#string"/>
  </owl:DatatypeProperty>
  <owl:DatatypeProperty rdf:about="http://example.org/onto/prop/google_gkeonprem_bare_metal_admin_cluster_no_proxy">
    <rdfs:label>no_proxy</rdfs:label>
    <rdfs:comment>A list of IPs, hostnames, and domains that should skip the proxy.
For example: ["127.0.0.1", "example.com", ".corp", "localhost"].</rdfs:comment>
    <rdfs:domain rdf:resource="http://example.org/onto/class/google_gkeonprem_bare_metal_admin_cluster"/>
    <rdfs:range rdf:resource="http://www.w3.org/2001/XMLSchema#string"/>
  </owl:DatatypeProperty>
  <owl:DatatypeProperty rdf:about="http://example.org/onto/prop/google_gkeonprem_bare_metal_admin_cluster_uri">
    <rdfs:label>uri</rdfs:label>
    <rdfs:comment>Specifies the address of your proxy server.
For Example: http://domain
WARNING: Do not provide credentials in the format
of http://(username:password@)domain these will be rejected by the server.</rdfs:comment>
    <rdfs:domain rdf:resource="http://example.org/onto/class/google_gkeonprem_bare_metal_admin_cluster"/>
    <rdfs:range rdf:resource="http://www.w3.org/2001/XMLSchema#string"/>
  </owl:DatatypeProperty>
  <owl:DatatypeProperty rdf:about="http://example.org/onto/prop/google_gkeonprem_bare_metal_admin_cluster_username">
    <rdfs:label>username</rdfs:label>
    <rdfs:comment>The name of the user, e.g. 'my-gcp-id@gmail.com'.</rdfs:comment>
    <rdfs:domain rdf:resource="http://example.org/onto/class/google_gkeonprem_bare_metal_admin_cluster"/>
    <rdfs:range rdf:resource="http://www.w3.org/2001/XMLSchema#string"/>
  </owl:DatatypeProperty>
  <owl:DatatypeProperty rdf:about="http://example.org/onto/prop/google_gkeonprem_bare_metal_admin_cluster_path">
    <rdfs:label>path</rdfs:label>
    <rdfs:comment>The host machine path.</rdfs:comment>
    <rdfs:domain rdf:resource="http://example.org/onto/class/google_gkeonprem_bare_metal_admin_cluster"/>
    <rdfs:range rdf:resource="http://www.w3.org/2001/XMLSchema#string"/>
  </owl:DatatypeProperty>
  <owl:DatatypeProperty rdf:about="http://example.org/onto/prop/google_gkeonprem_bare_metal_admin_cluster_storage_class">
    <rdfs:label>storage_class</rdfs:label>
    <rdfs:comment>The StorageClass name that PVs will be created with.</rdfs:comment>
    <rdfs:domain rdf:resource="http://example.org/onto/class/google_gkeonprem_bare_metal_admin_cluster"/>
    <rdfs:range rdf:resource="http://www.w3.org/2001/XMLSchema#string"/>
  </owl:DatatypeProperty>
  <owl:DatatypeProperty rdf:about="http://example.org/onto/prop/google_gkeonprem_bare_metal_admin_cluster_shared_path_pv_count">
    <rdfs:label>shared_path_pv_count</rdfs:label>
    <rdfs:comment>The number of subdirectories to create under path.</rdfs:comment>
    <rdfs:domain rdf:resource="http://example.org/onto/class/google_gkeonprem_bare_metal_admin_cluster"/>
    <rdfs:range rdf:resource="http://www.w3.org/2001/XMLSchema#string"/>
  </owl:DatatypeProperty>
  <owl:DatatypeProperty rdf:about="http://example.org/onto/prop/google_gkeonprem_bare_metal_admin_cluster_path">
    <rdfs:label>path</rdfs:label>
    <rdfs:comment>The host machine path.</rdfs:comment>
    <rdfs:domain rdf:resource="http://example.org/onto/class/google_gkeonprem_bare_metal_admin_cluster"/>
    <rdfs:range rdf:resource="http://www.w3.org/2001/XMLSchema#string"/>
  </owl:DatatypeProperty>
  <owl:DatatypeProperty rdf:about="http://example.org/onto/prop/google_gkeonprem_bare_metal_admin_cluster_storage_class">
    <rdfs:label>storage_class</rdfs:label>
    <rdfs:comment>The StorageClass name that PVs will be created with.</rdfs:comment>
    <rdfs:domain rdf:resource="http://example.org/onto/class/google_gkeonprem_bare_metal_admin_cluster"/>
    <rdfs:range rdf:resource="http://www.w3.org/2001/XMLSchema#string"/>
  </owl:DatatypeProperty>
  <owl:DatatypeProperty rdf:about="http://example.org/onto/prop/google_gkeonprem_bare_metal_admin_cluster_create">
    <rdfs:label>create</rdfs:label>
    <rdfs:domain rdf:resource="http://example.org/onto/class/google_gkeonprem_bare_metal_admin_cluster"/>
    <rdfs:range rdf:resource="http://www.w3.org/2001/XMLSchema#string"/>
  </owl:DatatypeProperty>
  <owl:DatatypeProperty rdf:about="http://example.org/onto/prop/google_gkeonprem_bare_metal_admin_cluster_delete">
    <rdfs:label>delete</rdfs:label>
    <rdfs:domain rdf:resource="http://example.org/onto/class/google_gkeonprem_bare_metal_admin_cluster"/>
    <rdfs:range rdf:resource="http://www.w3.org/2001/XMLSchema#string"/>
  </owl:DatatypeProperty>
  <owl:DatatypeProperty rdf:about="http://example.org/onto/prop/google_gkeonprem_bare_metal_admin_cluster_update">
    <rdfs:label>update</rdfs:label>
    <rdfs:domain rdf:resource="http://example.org/onto/class/google_gkeonprem_bare_metal_admin_cluster"/>
    <rdfs:range rdf:resource="http://www.w3.org/2001/XMLSchema#string"/>
  </owl:DatatypeProperty>
</rdf:RDF>
