<?xml version="1.0" encoding="UTF-8"?>
<rdf:RDF
  xmlns:rdf="http://www.w3.org/1999/02/22-rdf-syntax-ns#"
  xmlns:rdfs="http://www.w3.org/2000/01/rdf-schema#"
  xmlns:owl="http://www.w3.org/2002/07/owl#"
  xmlns:xsd="http://www.w3.org/2001/XMLSchema#"
  xml:base="http://example.org/onto/">
  <owl:Class rdf:about="http://example.org/onto/class/google_iap_settings">
    <rdfs:label>google_iap_settings</rdfs:label>
    <rdfs:comment>#
#     ***     AUTO GENERATED CODE    ***    Type: MMv1     ***
#
# ----------------------------------------------------------------------------
#
#     This code is generated by Magic Modules using the following:
#
#     Configuration: https:#github.com/GoogleCloudPlatform/magic-modules/tree/main/mmv1/products/iap/Settings.yaml
#     Template:      https:#github.com/GoogleCloudPlatform/magic-modules/tree/main/mmv1/templates/terraform/resource.html.markdown.tmpl
#
#     DO NOT EDIT this file directly. Any changes made to this file will be
#     overwritten during the next generation cycle.
#
# ----------------------------------------------------------------------------
subcategory: "Identity-Aware Proxy"
description: |-
  IAP settings - manage IAP settings
---</rdfs:comment>
  </owl:Class>
  <owl:DatatypeProperty rdf:about="http://example.org/onto/prop/google_iap_settings_id">
    <rdfs:label>id</rdfs:label>
    <rdfs:domain rdf:resource="http://example.org/onto/class/google_iap_settings"/>
    <rdfs:range rdf:resource="http://www.w3.org/2001/XMLSchema#string"/>
  </owl:DatatypeProperty>
  <owl:DatatypeProperty rdf:about="http://example.org/onto/prop/google_iap_settings_name">
    <rdfs:label>name</rdfs:label>
    <rdfs:comment>The resource name of the IAP protected resource. Name can have below resources:
* organizations/{organization_id}
* folders/{folder_id}
* projects/{project_id}
* projects/{project_id}/iap_web
* projects/{project_id}/iap_web/compute
* projects/{project_id}/iap_web/compute-{region}
* projects/{project_id}/iap_web/compute/services/{service_id}
* projects/{project_id}/iap_web/compute-{region}/services/{service_id}
* projects/{project_id}/iap_web/appengine-{app_id}
* projects/{project_id}/iap_web/appengine-{app_id}/services/{service_id}
* projects/{project_id}/iap_web/appengine-{app_id}/services/{service_id}/version/{version_id}</rdfs:comment>
    <rdfs:domain rdf:resource="http://example.org/onto/class/google_iap_settings"/>
    <rdfs:range rdf:resource="http://www.w3.org/2001/XMLSchema#string"/>
  </owl:DatatypeProperty>
  <owl:DatatypeProperty rdf:about="http://example.org/onto/prop/google_iap_settings_identity_sources">
    <rdfs:label>identity_sources</rdfs:label>
    <rdfs:comment>Identity sources that IAP can use to authenticate the end user. Only one identity source
can be configured. The possible values are:

* 'WORKFORCE_IDENTITY_FEDERATION': Use external identities set up on Google Cloud Workforce
  				     Identity Federation. Possible values: ["WORKFORCE_IDENTITY_FEDERATION"]</rdfs:comment>
    <rdfs:domain rdf:resource="http://example.org/onto/class/google_iap_settings"/>
    <rdfs:range rdf:resource="http://www.w3.org/2001/XMLSchema#string"/>
  </owl:DatatypeProperty>
  <owl:DatatypeProperty rdf:about="http://example.org/onto/prop/google_iap_settings_domains">
    <rdfs:label>domains</rdfs:label>
    <rdfs:comment>List of trusted domains.</rdfs:comment>
    <rdfs:domain rdf:resource="http://example.org/onto/class/google_iap_settings"/>
    <rdfs:range rdf:resource="http://www.w3.org/2001/XMLSchema#string"/>
  </owl:DatatypeProperty>
  <owl:DatatypeProperty rdf:about="http://example.org/onto/prop/google_iap_settings_enable">
    <rdfs:label>enable</rdfs:label>
    <rdfs:comment>Configuration for customers to opt in for the feature.</rdfs:comment>
    <rdfs:domain rdf:resource="http://example.org/onto/class/google_iap_settings"/>
    <rdfs:range rdf:resource="http://www.w3.org/2001/XMLSchema#string"/>
  </owl:DatatypeProperty>
  <owl:DatatypeProperty rdf:about="http://example.org/onto/prop/google_iap_settings_allow_http_options">
    <rdfs:label>allow_http_options</rdfs:label>
    <rdfs:comment>Configuration to allow HTTP OPTIONS calls to skip authorization.
If undefined, IAP will not apply any special logic to OPTIONS requests.</rdfs:comment>
    <rdfs:domain rdf:resource="http://example.org/onto/class/google_iap_settings"/>
    <rdfs:range rdf:resource="http://www.w3.org/2001/XMLSchema#string"/>
  </owl:DatatypeProperty>
  <owl:DatatypeProperty rdf:about="http://example.org/onto/prop/google_iap_settings_login_page_uri">
    <rdfs:label>login_page_uri</rdfs:label>
    <rdfs:comment>Login page URI associated with the GCIP tenants. Typically, all resources within
the same project share the same login page, though it could be overridden at the
sub resource level.</rdfs:comment>
    <rdfs:domain rdf:resource="http://example.org/onto/class/google_iap_settings"/>
    <rdfs:range rdf:resource="http://www.w3.org/2001/XMLSchema#string"/>
  </owl:DatatypeProperty>
  <owl:DatatypeProperty rdf:about="http://example.org/onto/prop/google_iap_settings_tenant_ids">
    <rdfs:label>tenant_ids</rdfs:label>
    <rdfs:comment>GCIP tenant ids that are linked to the IAP resource. tenantIds could be a string
beginning with a number character to indicate authenticating with GCIP tenant flow,
or in the format of _ to indicate authenticating with GCIP agent flow. If agent flow
is used, tenantIds should only contain one single element, while for tenant flow,
tenantIds can contain multiple elements.</rdfs:comment>
    <rdfs:domain rdf:resource="http://example.org/onto/class/google_iap_settings"/>
    <rdfs:range rdf:resource="http://www.w3.org/2001/XMLSchema#string"/>
  </owl:DatatypeProperty>
  <owl:DatatypeProperty rdf:about="http://example.org/onto/prop/google_iap_settings_login_hint">
    <rdfs:label>login_hint</rdfs:label>
    <rdfs:comment>Domain hint to send as hd=? parameter in OAuth request flow.
Enables redirect to primary IDP by skipping Google's login screen.
(https://developers.google.com/identity/protocols/OpenIDConnect#hd-param)
Note: IAP does not verify that the id token's hd claim matches this value
since access behavior is managed by IAM policies.
* loginHint setting is not a replacement for access control. Always enforce an appropriate access policy if you want to restrict access to users outside your domain.</rdfs:comment>
    <rdfs:domain rdf:resource="http://example.org/onto/class/google_iap_settings"/>
    <rdfs:range rdf:resource="http://www.w3.org/2001/XMLSchema#string"/>
  </owl:DatatypeProperty>
  <owl:DatatypeProperty rdf:about="http://example.org/onto/prop/google_iap_settings_programmatic_clients">
    <rdfs:label>programmatic_clients</rdfs:label>
    <rdfs:comment>List of client ids allowed to use IAP programmatically.</rdfs:comment>
    <rdfs:domain rdf:resource="http://example.org/onto/class/google_iap_settings"/>
    <rdfs:range rdf:resource="http://www.w3.org/2001/XMLSchema#string"/>
  </owl:DatatypeProperty>
  <owl:DatatypeProperty rdf:about="http://example.org/onto/prop/google_iap_settings_max_age">
    <rdfs:label>max_age</rdfs:label>
    <rdfs:comment>Reauth session lifetime, how long before a user has to reauthenticate again.
A duration in seconds with up to nine fractional digits, ending with 's'.
Example: "3.5s".</rdfs:comment>
    <rdfs:domain rdf:resource="http://example.org/onto/class/google_iap_settings"/>
    <rdfs:range rdf:resource="http://www.w3.org/2001/XMLSchema#string"/>
  </owl:DatatypeProperty>
  <owl:DatatypeProperty rdf:about="http://example.org/onto/prop/google_iap_settings_method">
    <rdfs:label>method</rdfs:label>
    <rdfs:comment>Reauth method requested. The possible values are:

* 'LOGIN': Prompts the user to log in again.
* 'SECURE_KEY': User must use their secure key 2nd factor device.
* 'ENROLLED_SECOND_FACTORS': User can use any enabled 2nd factor. Possible values: ["LOGIN", "SECURE_KEY", "ENROLLED_SECOND_FACTORS"]</rdfs:comment>
    <rdfs:domain rdf:resource="http://example.org/onto/class/google_iap_settings"/>
    <rdfs:range rdf:resource="http://www.w3.org/2001/XMLSchema#string"/>
  </owl:DatatypeProperty>
  <owl:DatatypeProperty rdf:about="http://example.org/onto/prop/google_iap_settings_policy_type">
    <rdfs:label>policy_type</rdfs:label>
    <rdfs:comment>How IAP determines the effective policy in cases of hierarchical policies.
Policies are merged from higher in the hierarchy to lower in the hierarchy.
The possible values are:

* 'MINIMUM': This policy acts as a minimum to other policies, lower in the hierarchy.
		   Effective policy may only be the same or stricter.
* 'DEFAULT': This policy acts as a default if no other reauth policy is set. Possible values: ["MINIMUM", "DEFAULT"]</rdfs:comment>
    <rdfs:domain rdf:resource="http://example.org/onto/class/google_iap_settings"/>
    <rdfs:range rdf:resource="http://www.w3.org/2001/XMLSchema#string"/>
  </owl:DatatypeProperty>
  <owl:DatatypeProperty rdf:about="http://example.org/onto/prop/google_iap_settings_workforce_pools">
    <rdfs:label>workforce_pools</rdfs:label>
    <rdfs:comment>The workforce pool resources. Only one workforce pool is accepted.</rdfs:comment>
    <rdfs:domain rdf:resource="http://example.org/onto/class/google_iap_settings"/>
    <rdfs:range rdf:resource="http://www.w3.org/2001/XMLSchema#string"/>
  </owl:DatatypeProperty>
  <owl:DatatypeProperty rdf:about="http://example.org/onto/prop/google_iap_settings_client_id">
    <rdfs:label>client_id</rdfs:label>
    <rdfs:comment>The OAuth 2.0 client ID registered in the workforce identity
federation OAuth 2.0 Server.</rdfs:comment>
    <rdfs:domain rdf:resource="http://example.org/onto/class/google_iap_settings"/>
    <rdfs:range rdf:resource="http://www.w3.org/2001/XMLSchema#string"/>
  </owl:DatatypeProperty>
  <owl:DatatypeProperty rdf:about="http://example.org/onto/prop/google_iap_settings_client_secret">
    <rdfs:label>client_secret</rdfs:label>
    <rdfs:comment>Input only. The OAuth 2.0 client secret created while registering
the client ID.</rdfs:comment>
    <rdfs:domain rdf:resource="http://example.org/onto/class/google_iap_settings"/>
    <rdfs:range rdf:resource="http://www.w3.org/2001/XMLSchema#string"/>
  </owl:DatatypeProperty>
  <owl:DatatypeProperty rdf:about="http://example.org/onto/prop/google_iap_settings_client_secret_sha256">
    <rdfs:label>client_secret_sha256</rdfs:label>
    <rdfs:comment>Output only. SHA256 hash value for the client secret. This field
is returned by IAP when the settings are retrieved.</rdfs:comment>
    <rdfs:domain rdf:resource="http://example.org/onto/class/google_iap_settings"/>
    <rdfs:range rdf:resource="http://www.w3.org/2001/XMLSchema#string"/>
  </owl:DatatypeProperty>
  <owl:DatatypeProperty rdf:about="http://example.org/onto/prop/google_iap_settings_cookie_domain">
    <rdfs:label>cookie_domain</rdfs:label>
    <rdfs:comment>The Domain value to set for cookies generated by IAP. This value is not validated by the API,
but will be ignored at runtime if invalid.</rdfs:comment>
    <rdfs:domain rdf:resource="http://example.org/onto/class/google_iap_settings"/>
    <rdfs:range rdf:resource="http://www.w3.org/2001/XMLSchema#string"/>
  </owl:DatatypeProperty>
  <owl:DatatypeProperty rdf:about="http://example.org/onto/prop/google_iap_settings_access_denied_page_uri">
    <rdfs:label>access_denied_page_uri</rdfs:label>
    <rdfs:comment>The URI to be redirected to when access is denied.</rdfs:comment>
    <rdfs:domain rdf:resource="http://example.org/onto/class/google_iap_settings"/>
    <rdfs:range rdf:resource="http://www.w3.org/2001/XMLSchema#string"/>
  </owl:DatatypeProperty>
  <owl:DatatypeProperty rdf:about="http://example.org/onto/prop/google_iap_settings_generate_troubleshooting_uri">
    <rdfs:label>generate_troubleshooting_uri</rdfs:label>
    <rdfs:comment>Whether to generate a troubleshooting URL on access denied events to this application.</rdfs:comment>
    <rdfs:domain rdf:resource="http://example.org/onto/class/google_iap_settings"/>
    <rdfs:range rdf:resource="http://www.w3.org/2001/XMLSchema#string"/>
  </owl:DatatypeProperty>
  <owl:DatatypeProperty rdf:about="http://example.org/onto/prop/google_iap_settings_remediation_token_generation_enabled">
    <rdfs:label>remediation_token_generation_enabled</rdfs:label>
    <rdfs:comment>Whether to generate remediation token on access denied events to this application.</rdfs:comment>
    <rdfs:domain rdf:resource="http://example.org/onto/class/google_iap_settings"/>
    <rdfs:range rdf:resource="http://www.w3.org/2001/XMLSchema#string"/>
  </owl:DatatypeProperty>
  <owl:DatatypeProperty rdf:about="http://example.org/onto/prop/google_iap_settings_enable">
    <rdfs:label>enable</rdfs:label>
    <rdfs:comment>Whether the provided attribute propagation settings should be evaluated on user requests.
If set to true, attributes returned from the expression will be propagated in the set output credentials.</rdfs:comment>
    <rdfs:domain rdf:resource="http://example.org/onto/class/google_iap_settings"/>
    <rdfs:range rdf:resource="http://www.w3.org/2001/XMLSchema#string"/>
  </owl:DatatypeProperty>
  <owl:DatatypeProperty rdf:about="http://example.org/onto/prop/google_iap_settings_expression">
    <rdfs:label>expression</rdfs:label>
    <rdfs:comment>Raw string CEL expression. Must return a list of attributes. A maximum of 45 attributes can
be selected. Expressions can select different attribute types from attributes:
attributes.saml_attributes, attributes.iap_attributes.</rdfs:comment>
    <rdfs:domain rdf:resource="http://example.org/onto/class/google_iap_settings"/>
    <rdfs:range rdf:resource="http://www.w3.org/2001/XMLSchema#string"/>
  </owl:DatatypeProperty>
  <owl:DatatypeProperty rdf:about="http://example.org/onto/prop/google_iap_settings_output_credentials">
    <rdfs:label>output_credentials</rdfs:label>
    <rdfs:comment>Which output credentials attributes selected by the CEL expression should be propagated in.
All attributes will be fully duplicated in each selected output credential.
Possible values are:

* 'HEADER': Propagate attributes in the headers with "x-goog-iap-attr-" prefix.
* 'JWT': Propagate attributes in the JWT of the form:
         "additional_claims": { "my_attribute": ["value1", "value2"] }
* 'RCTOKEN': Propagate attributes in the RCToken of the form: "
             additional_claims": { "my_attribute": ["value1", "value2"] } Possible values: ["HEADER", "JWT", "RCTOKEN"]</rdfs:comment>
    <rdfs:domain rdf:resource="http://example.org/onto/class/google_iap_settings"/>
    <rdfs:range rdf:resource="http://www.w3.org/2001/XMLSchema#string"/>
  </owl:DatatypeProperty>
  <owl:DatatypeProperty rdf:about="http://example.org/onto/prop/google_iap_settings_rctoken_aud">
    <rdfs:label>rctoken_aud</rdfs:label>
    <rdfs:comment>Audience claim set in the generated RCToken. This value is not validated by IAP.</rdfs:comment>
    <rdfs:domain rdf:resource="http://example.org/onto/class/google_iap_settings"/>
    <rdfs:range rdf:resource="http://www.w3.org/2001/XMLSchema#string"/>
  </owl:DatatypeProperty>
  <owl:DatatypeProperty rdf:about="http://example.org/onto/prop/google_iap_settings_create">
    <rdfs:label>create</rdfs:label>
    <rdfs:domain rdf:resource="http://example.org/onto/class/google_iap_settings"/>
    <rdfs:range rdf:resource="http://www.w3.org/2001/XMLSchema#string"/>
  </owl:DatatypeProperty>
  <owl:DatatypeProperty rdf:about="http://example.org/onto/prop/google_iap_settings_delete">
    <rdfs:label>delete</rdfs:label>
    <rdfs:domain rdf:resource="http://example.org/onto/class/google_iap_settings"/>
    <rdfs:range rdf:resource="http://www.w3.org/2001/XMLSchema#string"/>
  </owl:DatatypeProperty>
  <owl:DatatypeProperty rdf:about="http://example.org/onto/prop/google_iap_settings_update">
    <rdfs:label>update</rdfs:label>
    <rdfs:domain rdf:resource="http://example.org/onto/class/google_iap_settings"/>
    <rdfs:range rdf:resource="http://www.w3.org/2001/XMLSchema#string"/>
  </owl:DatatypeProperty>
</rdf:RDF>
