<?xml version="1.0" encoding="UTF-8"?>
<rdf:RDF
  xmlns:rdf="http://www.w3.org/1999/02/22-rdf-syntax-ns#"
  xmlns:rdfs="http://www.w3.org/2000/01/rdf-schema#"
  xmlns:owl="http://www.w3.org/2002/07/owl#"
  xmlns:xsd="http://www.w3.org/2001/XMLSchema#"
  xml:base="http://example.org/onto/">
  <owl:Class rdf:about="http://example.org/onto/class/google_apigee_developer_app">
    <rdfs:label>google_apigee_developer_app</rdfs:label>
    <rdfs:comment>#
#     ***     AUTO GENERATED CODE    ***    Type: MMv1     ***
#
# ----------------------------------------------------------------------------
#
#     This code is generated by Magic Modules using the following:
#
#     Configuration: https:#github.com/GoogleCloudPlatform/magic-modules/tree/main/mmv1/products/apigee/DeveloperApp.yaml
#     Template:      https:#github.com/GoogleCloudPlatform/magic-modules/tree/main/mmv1/templates/terraform/resource.html.markdown.tmpl
#
#     DO NOT EDIT this file directly. Any changes made to this file will be
#     overwritten during the next generation cycle.
#
# ----------------------------------------------------------------------------
subcategory: "Apigee"
description: |-
  Creates an app associated with a developer.
---</rdfs:comment>
  </owl:Class>
  <owl:DatatypeProperty rdf:about="http://example.org/onto/prop/google_apigee_developer_app_api_products">
    <rdfs:label>api_products</rdfs:label>
    <rdfs:comment>List of API products associated with the developer app.</rdfs:comment>
    <rdfs:domain rdf:resource="http://example.org/onto/class/google_apigee_developer_app"/>
    <rdfs:range rdf:resource="http://www.w3.org/2001/XMLSchema#string"/>
  </owl:DatatypeProperty>
  <owl:DatatypeProperty rdf:about="http://example.org/onto/prop/google_apigee_developer_app_app_family">
    <rdfs:label>app_family</rdfs:label>
    <rdfs:comment>Developer app family.</rdfs:comment>
    <rdfs:domain rdf:resource="http://example.org/onto/class/google_apigee_developer_app"/>
    <rdfs:range rdf:resource="http://www.w3.org/2001/XMLSchema#string"/>
  </owl:DatatypeProperty>
  <owl:DatatypeProperty rdf:about="http://example.org/onto/prop/google_apigee_developer_app_app_id">
    <rdfs:label>app_id</rdfs:label>
    <rdfs:comment>ID of the developer app. This ID is not user specified but is
automatically generated on app creation. appId is a UUID.</rdfs:comment>
    <rdfs:domain rdf:resource="http://example.org/onto/class/google_apigee_developer_app"/>
    <rdfs:range rdf:resource="http://www.w3.org/2001/XMLSchema#string"/>
  </owl:DatatypeProperty>
  <owl:DatatypeProperty rdf:about="http://example.org/onto/prop/google_apigee_developer_app_callback_url">
    <rdfs:label>callback_url</rdfs:label>
    <rdfs:comment>Callback URL used by OAuth 2.0 authorization servers to communicate
authorization codes back to developer apps.</rdfs:comment>
    <rdfs:domain rdf:resource="http://example.org/onto/class/google_apigee_developer_app"/>
    <rdfs:range rdf:resource="http://www.w3.org/2001/XMLSchema#string"/>
  </owl:DatatypeProperty>
  <owl:DatatypeProperty rdf:about="http://example.org/onto/prop/google_apigee_developer_app_created_at">
    <rdfs:label>created_at</rdfs:label>
    <rdfs:comment>Time at which the developer was created in milliseconds since epoch.</rdfs:comment>
    <rdfs:domain rdf:resource="http://example.org/onto/class/google_apigee_developer_app"/>
    <rdfs:range rdf:resource="http://www.w3.org/2001/XMLSchema#string"/>
  </owl:DatatypeProperty>
  <owl:DatatypeProperty rdf:about="http://example.org/onto/prop/google_apigee_developer_app_credentials">
    <rdfs:label>credentials</rdfs:label>
    <rdfs:comment>Output only. Set of credentials for the developer app consisting of
the consumer key/secret pairs associated with the API products.</rdfs:comment>
    <rdfs:domain rdf:resource="http://example.org/onto/class/google_apigee_developer_app"/>
    <rdfs:range rdf:resource="http://www.w3.org/2001/XMLSchema#string"/>
  </owl:DatatypeProperty>
  <owl:DatatypeProperty rdf:about="http://example.org/onto/prop/google_apigee_developer_app_developer_email">
    <rdfs:label>developer_email</rdfs:label>
    <rdfs:comment>Email address of the developer.
This value is used to uniquely identify the developer in Apigee hybrid.
Note that the email address has to be in lowercase only.</rdfs:comment>
    <rdfs:domain rdf:resource="http://example.org/onto/class/google_apigee_developer_app"/>
    <rdfs:range rdf:resource="http://www.w3.org/2001/XMLSchema#string"/>
  </owl:DatatypeProperty>
  <owl:DatatypeProperty rdf:about="http://example.org/onto/prop/google_apigee_developer_app_developer_id">
    <rdfs:label>developer_id</rdfs:label>
    <rdfs:comment>ID of the developer.</rdfs:comment>
    <rdfs:domain rdf:resource="http://example.org/onto/class/google_apigee_developer_app"/>
    <rdfs:range rdf:resource="http://www.w3.org/2001/XMLSchema#string"/>
  </owl:DatatypeProperty>
  <owl:DatatypeProperty rdf:about="http://example.org/onto/prop/google_apigee_developer_app_id">
    <rdfs:label>id</rdfs:label>
    <rdfs:domain rdf:resource="http://example.org/onto/class/google_apigee_developer_app"/>
    <rdfs:range rdf:resource="http://www.w3.org/2001/XMLSchema#string"/>
  </owl:DatatypeProperty>
  <owl:DatatypeProperty rdf:about="http://example.org/onto/prop/google_apigee_developer_app_key_expires_in">
    <rdfs:label>key_expires_in</rdfs:label>
    <rdfs:comment>Expiration time, in milliseconds, for the consumer key that is generated
for the developer app. If not set or left to the default value of -1,
the API key never expires. The expiration time can't be updated after it is set.</rdfs:comment>
    <rdfs:domain rdf:resource="http://example.org/onto/class/google_apigee_developer_app"/>
    <rdfs:range rdf:resource="http://www.w3.org/2001/XMLSchema#string"/>
  </owl:DatatypeProperty>
  <owl:DatatypeProperty rdf:about="http://example.org/onto/prop/google_apigee_developer_app_last_modified_at">
    <rdfs:label>last_modified_at</rdfs:label>
    <rdfs:comment>Time at which the developer was last modified in milliseconds since epoch.</rdfs:comment>
    <rdfs:domain rdf:resource="http://example.org/onto/class/google_apigee_developer_app"/>
    <rdfs:range rdf:resource="http://www.w3.org/2001/XMLSchema#string"/>
  </owl:DatatypeProperty>
  <owl:DatatypeProperty rdf:about="http://example.org/onto/prop/google_apigee_developer_app_name">
    <rdfs:label>name</rdfs:label>
    <rdfs:comment>Name of the developer app.</rdfs:comment>
    <rdfs:domain rdf:resource="http://example.org/onto/class/google_apigee_developer_app"/>
    <rdfs:range rdf:resource="http://www.w3.org/2001/XMLSchema#string"/>
  </owl:DatatypeProperty>
  <owl:DatatypeProperty rdf:about="http://example.org/onto/prop/google_apigee_developer_app_org_id">
    <rdfs:label>org_id</rdfs:label>
    <rdfs:comment>The Apigee Organization associated with the Apigee instance,
in the format 'organizations/{{org_name}}'.</rdfs:comment>
    <rdfs:domain rdf:resource="http://example.org/onto/class/google_apigee_developer_app"/>
    <rdfs:range rdf:resource="http://www.w3.org/2001/XMLSchema#string"/>
  </owl:DatatypeProperty>
  <owl:DatatypeProperty rdf:about="http://example.org/onto/prop/google_apigee_developer_app_scopes">
    <rdfs:label>scopes</rdfs:label>
    <rdfs:comment>Scopes to apply to the developer app.
The specified scopes must already exist for the API product that
you associate with the developer app.</rdfs:comment>
    <rdfs:domain rdf:resource="http://example.org/onto/class/google_apigee_developer_app"/>
    <rdfs:range rdf:resource="http://www.w3.org/2001/XMLSchema#string"/>
  </owl:DatatypeProperty>
  <owl:DatatypeProperty rdf:about="http://example.org/onto/prop/google_apigee_developer_app_status">
    <rdfs:label>status</rdfs:label>
    <rdfs:comment>Status of the credential. Valid values include approved or revoked.</rdfs:comment>
    <rdfs:domain rdf:resource="http://example.org/onto/class/google_apigee_developer_app"/>
    <rdfs:range rdf:resource="http://www.w3.org/2001/XMLSchema#string"/>
  </owl:DatatypeProperty>
  <owl:DatatypeProperty rdf:about="http://example.org/onto/prop/google_apigee_developer_app_name">
    <rdfs:label>name</rdfs:label>
    <rdfs:comment>Key of the attribute</rdfs:comment>
    <rdfs:domain rdf:resource="http://example.org/onto/class/google_apigee_developer_app"/>
    <rdfs:range rdf:resource="http://www.w3.org/2001/XMLSchema#string"/>
  </owl:DatatypeProperty>
  <owl:DatatypeProperty rdf:about="http://example.org/onto/prop/google_apigee_developer_app_value">
    <rdfs:label>value</rdfs:label>
    <rdfs:comment>Value of the attribute</rdfs:comment>
    <rdfs:domain rdf:resource="http://example.org/onto/class/google_apigee_developer_app"/>
    <rdfs:range rdf:resource="http://www.w3.org/2001/XMLSchema#string"/>
  </owl:DatatypeProperty>
  <owl:DatatypeProperty rdf:about="http://example.org/onto/prop/google_apigee_developer_app_create">
    <rdfs:label>create</rdfs:label>
    <rdfs:domain rdf:resource="http://example.org/onto/class/google_apigee_developer_app"/>
    <rdfs:range rdf:resource="http://www.w3.org/2001/XMLSchema#string"/>
  </owl:DatatypeProperty>
  <owl:DatatypeProperty rdf:about="http://example.org/onto/prop/google_apigee_developer_app_delete">
    <rdfs:label>delete</rdfs:label>
    <rdfs:domain rdf:resource="http://example.org/onto/class/google_apigee_developer_app"/>
    <rdfs:range rdf:resource="http://www.w3.org/2001/XMLSchema#string"/>
  </owl:DatatypeProperty>
  <owl:DatatypeProperty rdf:about="http://example.org/onto/prop/google_apigee_developer_app_update">
    <rdfs:label>update</rdfs:label>
    <rdfs:domain rdf:resource="http://example.org/onto/class/google_apigee_developer_app"/>
    <rdfs:range rdf:resource="http://www.w3.org/2001/XMLSchema#string"/>
  </owl:DatatypeProperty>
</rdf:RDF>
