<?xml version="1.0" encoding="UTF-8"?>
<rdf:RDF
  xmlns:rdf="http://www.w3.org/1999/02/22-rdf-syntax-ns#"
  xmlns:rdfs="http://www.w3.org/2000/01/rdf-schema#"
  xmlns:owl="http://www.w3.org/2002/07/owl#"
  xmlns:xsd="http://www.w3.org/2001/XMLSchema#"
  xml:base="http://example.org/onto/">
  <owl:Class rdf:about="http://example.org/onto/class/google_cloudfunctions2_function">
    <rdfs:label>google_cloudfunctions2_function</rdfs:label>
    <rdfs:comment>#
#     ***     AUTO GENERATED CODE    ***    Type: MMv1     ***
#
# ----------------------------------------------------------------------------
#
#     This code is generated by Magic Modules using the following:
#
#     Configuration: https:#github.com/GoogleCloudPlatform/magic-modules/tree/main/mmv1/products/cloudfunctions2/Function.yaml
#     Template:      https:#github.com/GoogleCloudPlatform/magic-modules/tree/main/mmv1/templates/terraform/resource.html.markdown.tmpl
#
#     DO NOT EDIT this file directly. Any changes made to this file will be
#     overwritten during the next generation cycle.
#
# ----------------------------------------------------------------------------
subcategory: "Cloud Functions (2nd gen)"
description: |-
  A Cloud Function that contains user computation executed in response to an event.
---</rdfs:comment>
  </owl:Class>
  <owl:DatatypeProperty rdf:about="http://example.org/onto/prop/google_cloudfunctions2_function_description">
    <rdfs:label>description</rdfs:label>
    <rdfs:comment>User-provided description of a function.</rdfs:comment>
    <rdfs:domain rdf:resource="http://example.org/onto/class/google_cloudfunctions2_function"/>
    <rdfs:range rdf:resource="http://www.w3.org/2001/XMLSchema#string"/>
  </owl:DatatypeProperty>
  <owl:DatatypeProperty rdf:about="http://example.org/onto/prop/google_cloudfunctions2_function_effective_labels">
    <rdfs:label>effective_labels</rdfs:label>
    <rdfs:comment>All of labels (key/value pairs) present on the resource in GCP, including the labels configured through Terraform, other clients and services.</rdfs:comment>
    <rdfs:domain rdf:resource="http://example.org/onto/class/google_cloudfunctions2_function"/>
    <rdfs:range rdf:resource="http://www.w3.org/2001/XMLSchema#string"/>
  </owl:DatatypeProperty>
  <owl:DatatypeProperty rdf:about="http://example.org/onto/prop/google_cloudfunctions2_function_environment">
    <rdfs:label>environment</rdfs:label>
    <rdfs:comment>The environment the function is hosted on.</rdfs:comment>
    <rdfs:domain rdf:resource="http://example.org/onto/class/google_cloudfunctions2_function"/>
    <rdfs:range rdf:resource="http://www.w3.org/2001/XMLSchema#string"/>
  </owl:DatatypeProperty>
  <owl:DatatypeProperty rdf:about="http://example.org/onto/prop/google_cloudfunctions2_function_id">
    <rdfs:label>id</rdfs:label>
    <rdfs:domain rdf:resource="http://example.org/onto/class/google_cloudfunctions2_function"/>
    <rdfs:range rdf:resource="http://www.w3.org/2001/XMLSchema#string"/>
  </owl:DatatypeProperty>
  <owl:DatatypeProperty rdf:about="http://example.org/onto/prop/google_cloudfunctions2_function_kms_key_name">
    <rdfs:label>kms_key_name</rdfs:label>
    <rdfs:comment>Resource name of a KMS crypto key (managed by the user) used to encrypt/decrypt function resources.
It must match the pattern projects/{project}/locations/{location}/keyRings/{key_ring}/cryptoKeys/{crypto_key}.</rdfs:comment>
    <rdfs:domain rdf:resource="http://example.org/onto/class/google_cloudfunctions2_function"/>
    <rdfs:range rdf:resource="http://www.w3.org/2001/XMLSchema#string"/>
  </owl:DatatypeProperty>
  <owl:DatatypeProperty rdf:about="http://example.org/onto/prop/google_cloudfunctions2_function_labels">
    <rdfs:label>labels</rdfs:label>
    <rdfs:comment>A set of key/value label pairs associated with this Cloud Function.


**Note**: This field is non-authoritative, and will only manage the labels present in your configuration.
Please refer to the field 'effective_labels' for all of the labels present on the resource.</rdfs:comment>
    <rdfs:domain rdf:resource="http://example.org/onto/class/google_cloudfunctions2_function"/>
    <rdfs:range rdf:resource="http://www.w3.org/2001/XMLSchema#string"/>
  </owl:DatatypeProperty>
  <owl:DatatypeProperty rdf:about="http://example.org/onto/prop/google_cloudfunctions2_function_location">
    <rdfs:label>location</rdfs:label>
    <rdfs:comment>The location of this cloud function.</rdfs:comment>
    <rdfs:domain rdf:resource="http://example.org/onto/class/google_cloudfunctions2_function"/>
    <rdfs:range rdf:resource="http://www.w3.org/2001/XMLSchema#string"/>
  </owl:DatatypeProperty>
  <owl:DatatypeProperty rdf:about="http://example.org/onto/prop/google_cloudfunctions2_function_name">
    <rdfs:label>name</rdfs:label>
    <rdfs:comment>A user-defined name of the function. Function names must
be unique globally and match pattern 'projects/*/locations/*/functions/*'.</rdfs:comment>
    <rdfs:domain rdf:resource="http://example.org/onto/class/google_cloudfunctions2_function"/>
    <rdfs:range rdf:resource="http://www.w3.org/2001/XMLSchema#string"/>
  </owl:DatatypeProperty>
  <owl:DatatypeProperty rdf:about="http://example.org/onto/prop/google_cloudfunctions2_function_project">
    <rdfs:label>project</rdfs:label>
    <rdfs:domain rdf:resource="http://example.org/onto/class/google_cloudfunctions2_function"/>
    <rdfs:range rdf:resource="http://www.w3.org/2001/XMLSchema#string"/>
  </owl:DatatypeProperty>
  <owl:DatatypeProperty rdf:about="http://example.org/onto/prop/google_cloudfunctions2_function_state">
    <rdfs:label>state</rdfs:label>
    <rdfs:comment>Describes the current state of the function.</rdfs:comment>
    <rdfs:domain rdf:resource="http://example.org/onto/class/google_cloudfunctions2_function"/>
    <rdfs:range rdf:resource="http://www.w3.org/2001/XMLSchema#string"/>
  </owl:DatatypeProperty>
  <owl:DatatypeProperty rdf:about="http://example.org/onto/prop/google_cloudfunctions2_function_terraform_labels">
    <rdfs:label>terraform_labels</rdfs:label>
    <rdfs:comment>The combination of labels configured directly on the resource
 and default labels configured on the provider.</rdfs:comment>
    <rdfs:domain rdf:resource="http://example.org/onto/class/google_cloudfunctions2_function"/>
    <rdfs:range rdf:resource="http://www.w3.org/2001/XMLSchema#string"/>
  </owl:DatatypeProperty>
  <owl:DatatypeProperty rdf:about="http://example.org/onto/prop/google_cloudfunctions2_function_update_time">
    <rdfs:label>update_time</rdfs:label>
    <rdfs:comment>The last update timestamp of a Cloud Function.</rdfs:comment>
    <rdfs:domain rdf:resource="http://example.org/onto/class/google_cloudfunctions2_function"/>
    <rdfs:range rdf:resource="http://www.w3.org/2001/XMLSchema#string"/>
  </owl:DatatypeProperty>
  <owl:DatatypeProperty rdf:about="http://example.org/onto/prop/google_cloudfunctions2_function_url">
    <rdfs:label>url</rdfs:label>
    <rdfs:comment>Output only. The deployed url for the function.</rdfs:comment>
    <rdfs:domain rdf:resource="http://example.org/onto/class/google_cloudfunctions2_function"/>
    <rdfs:range rdf:resource="http://www.w3.org/2001/XMLSchema#string"/>
  </owl:DatatypeProperty>
  <owl:DatatypeProperty rdf:about="http://example.org/onto/prop/google_cloudfunctions2_function_build">
    <rdfs:label>build</rdfs:label>
    <rdfs:comment>The Cloud Build name of the latest successful
deployment of the function.</rdfs:comment>
    <rdfs:domain rdf:resource="http://example.org/onto/class/google_cloudfunctions2_function"/>
    <rdfs:range rdf:resource="http://www.w3.org/2001/XMLSchema#string"/>
  </owl:DatatypeProperty>
  <owl:DatatypeProperty rdf:about="http://example.org/onto/prop/google_cloudfunctions2_function_docker_repository">
    <rdfs:label>docker_repository</rdfs:label>
    <rdfs:comment>User managed repository created in Artifact Registry optionally with a customer managed encryption key.</rdfs:comment>
    <rdfs:domain rdf:resource="http://example.org/onto/class/google_cloudfunctions2_function"/>
    <rdfs:range rdf:resource="http://www.w3.org/2001/XMLSchema#string"/>
  </owl:DatatypeProperty>
  <owl:DatatypeProperty rdf:about="http://example.org/onto/prop/google_cloudfunctions2_function_entry_point">
    <rdfs:label>entry_point</rdfs:label>
    <rdfs:comment>The name of the function (as defined in source code) that will be executed.
Defaults to the resource name suffix, if not specified. For backward
compatibility, if function with given name is not found, then the system
will try to use function named "function". For Node.js this is name of a
function exported by the module specified in source_location.</rdfs:comment>
    <rdfs:domain rdf:resource="http://example.org/onto/class/google_cloudfunctions2_function"/>
    <rdfs:range rdf:resource="http://www.w3.org/2001/XMLSchema#string"/>
  </owl:DatatypeProperty>
  <owl:DatatypeProperty rdf:about="http://example.org/onto/prop/google_cloudfunctions2_function_environment_variables">
    <rdfs:label>environment_variables</rdfs:label>
    <rdfs:comment>User-provided build-time environment variables for the function.</rdfs:comment>
    <rdfs:domain rdf:resource="http://example.org/onto/class/google_cloudfunctions2_function"/>
    <rdfs:range rdf:resource="http://www.w3.org/2001/XMLSchema#string"/>
  </owl:DatatypeProperty>
  <owl:DatatypeProperty rdf:about="http://example.org/onto/prop/google_cloudfunctions2_function_runtime">
    <rdfs:label>runtime</rdfs:label>
    <rdfs:comment>The runtime in which to run the function. Required when deploying a new
function, optional when updating an existing function.</rdfs:comment>
    <rdfs:domain rdf:resource="http://example.org/onto/class/google_cloudfunctions2_function"/>
    <rdfs:range rdf:resource="http://www.w3.org/2001/XMLSchema#string"/>
  </owl:DatatypeProperty>
  <owl:DatatypeProperty rdf:about="http://example.org/onto/prop/google_cloudfunctions2_function_service_account">
    <rdfs:label>service_account</rdfs:label>
    <rdfs:comment>The fully-qualified name of the service account to be used for building the container.</rdfs:comment>
    <rdfs:domain rdf:resource="http://example.org/onto/class/google_cloudfunctions2_function"/>
    <rdfs:range rdf:resource="http://www.w3.org/2001/XMLSchema#string"/>
  </owl:DatatypeProperty>
  <owl:DatatypeProperty rdf:about="http://example.org/onto/prop/google_cloudfunctions2_function_worker_pool">
    <rdfs:label>worker_pool</rdfs:label>
    <rdfs:comment>Name of the Cloud Build Custom Worker Pool that should be used to build the function.</rdfs:comment>
    <rdfs:domain rdf:resource="http://example.org/onto/class/google_cloudfunctions2_function"/>
    <rdfs:range rdf:resource="http://www.w3.org/2001/XMLSchema#string"/>
  </owl:DatatypeProperty>
  <owl:DatatypeProperty rdf:about="http://example.org/onto/prop/google_cloudfunctions2_function_runtime_version">
    <rdfs:label>runtime_version</rdfs:label>
    <rdfs:comment>The runtime version which was used during latest function deployment.</rdfs:comment>
    <rdfs:domain rdf:resource="http://example.org/onto/class/google_cloudfunctions2_function"/>
    <rdfs:range rdf:resource="http://www.w3.org/2001/XMLSchema#string"/>
  </owl:DatatypeProperty>
  <owl:DatatypeProperty rdf:about="http://example.org/onto/prop/google_cloudfunctions2_function_branch_name">
    <rdfs:label>branch_name</rdfs:label>
    <rdfs:comment>Regex matching branches to build.</rdfs:comment>
    <rdfs:domain rdf:resource="http://example.org/onto/class/google_cloudfunctions2_function"/>
    <rdfs:range rdf:resource="http://www.w3.org/2001/XMLSchema#string"/>
  </owl:DatatypeProperty>
  <owl:DatatypeProperty rdf:about="http://example.org/onto/prop/google_cloudfunctions2_function_commit_sha">
    <rdfs:label>commit_sha</rdfs:label>
    <rdfs:comment>Regex matching tags to build.</rdfs:comment>
    <rdfs:domain rdf:resource="http://example.org/onto/class/google_cloudfunctions2_function"/>
    <rdfs:range rdf:resource="http://www.w3.org/2001/XMLSchema#string"/>
  </owl:DatatypeProperty>
  <owl:DatatypeProperty rdf:about="http://example.org/onto/prop/google_cloudfunctions2_function_dir">
    <rdfs:label>dir</rdfs:label>
    <rdfs:comment>Directory, relative to the source root, in which to run the build.</rdfs:comment>
    <rdfs:domain rdf:resource="http://example.org/onto/class/google_cloudfunctions2_function"/>
    <rdfs:range rdf:resource="http://www.w3.org/2001/XMLSchema#string"/>
  </owl:DatatypeProperty>
  <owl:DatatypeProperty rdf:about="http://example.org/onto/prop/google_cloudfunctions2_function_invert_regex">
    <rdfs:label>invert_regex</rdfs:label>
    <rdfs:comment>Only trigger a build if the revision regex does
NOT match the revision regex.</rdfs:comment>
    <rdfs:domain rdf:resource="http://example.org/onto/class/google_cloudfunctions2_function"/>
    <rdfs:range rdf:resource="http://www.w3.org/2001/XMLSchema#string"/>
  </owl:DatatypeProperty>
  <owl:DatatypeProperty rdf:about="http://example.org/onto/prop/google_cloudfunctions2_function_project_id">
    <rdfs:label>project_id</rdfs:label>
    <rdfs:comment>ID of the project that owns the Cloud Source Repository. If omitted, the
project ID requesting the build is assumed.</rdfs:comment>
    <rdfs:domain rdf:resource="http://example.org/onto/class/google_cloudfunctions2_function"/>
    <rdfs:range rdf:resource="http://www.w3.org/2001/XMLSchema#string"/>
  </owl:DatatypeProperty>
  <owl:DatatypeProperty rdf:about="http://example.org/onto/prop/google_cloudfunctions2_function_repo_name">
    <rdfs:label>repo_name</rdfs:label>
    <rdfs:comment>Name of the Cloud Source Repository.</rdfs:comment>
    <rdfs:domain rdf:resource="http://example.org/onto/class/google_cloudfunctions2_function"/>
    <rdfs:range rdf:resource="http://www.w3.org/2001/XMLSchema#string"/>
  </owl:DatatypeProperty>
  <owl:DatatypeProperty rdf:about="http://example.org/onto/prop/google_cloudfunctions2_function_tag_name">
    <rdfs:label>tag_name</rdfs:label>
    <rdfs:comment>Regex matching tags to build.</rdfs:comment>
    <rdfs:domain rdf:resource="http://example.org/onto/class/google_cloudfunctions2_function"/>
    <rdfs:range rdf:resource="http://www.w3.org/2001/XMLSchema#string"/>
  </owl:DatatypeProperty>
  <owl:DatatypeProperty rdf:about="http://example.org/onto/prop/google_cloudfunctions2_function_bucket">
    <rdfs:label>bucket</rdfs:label>
    <rdfs:comment>Google Cloud Storage bucket containing the source</rdfs:comment>
    <rdfs:domain rdf:resource="http://example.org/onto/class/google_cloudfunctions2_function"/>
    <rdfs:range rdf:resource="http://www.w3.org/2001/XMLSchema#string"/>
  </owl:DatatypeProperty>
  <owl:DatatypeProperty rdf:about="http://example.org/onto/prop/google_cloudfunctions2_function_generation">
    <rdfs:label>generation</rdfs:label>
    <rdfs:comment>Google Cloud Storage generation for the object. If the generation
is omitted, the latest generation will be used.</rdfs:comment>
    <rdfs:domain rdf:resource="http://example.org/onto/class/google_cloudfunctions2_function"/>
    <rdfs:range rdf:resource="http://www.w3.org/2001/XMLSchema#string"/>
  </owl:DatatypeProperty>
  <owl:DatatypeProperty rdf:about="http://example.org/onto/prop/google_cloudfunctions2_function_object">
    <rdfs:label>object</rdfs:label>
    <rdfs:comment>Google Cloud Storage object containing the source.</rdfs:comment>
    <rdfs:domain rdf:resource="http://example.org/onto/class/google_cloudfunctions2_function"/>
    <rdfs:range rdf:resource="http://www.w3.org/2001/XMLSchema#string"/>
  </owl:DatatypeProperty>
  <owl:DatatypeProperty rdf:about="http://example.org/onto/prop/google_cloudfunctions2_function_event_type">
    <rdfs:label>event_type</rdfs:label>
    <rdfs:comment>Required. The type of event to observe.</rdfs:comment>
    <rdfs:domain rdf:resource="http://example.org/onto/class/google_cloudfunctions2_function"/>
    <rdfs:range rdf:resource="http://www.w3.org/2001/XMLSchema#string"/>
  </owl:DatatypeProperty>
  <owl:DatatypeProperty rdf:about="http://example.org/onto/prop/google_cloudfunctions2_function_pubsub_topic">
    <rdfs:label>pubsub_topic</rdfs:label>
    <rdfs:comment>The name of a Pub/Sub topic in the same project that will be used
as the transport topic for the event delivery.</rdfs:comment>
    <rdfs:domain rdf:resource="http://example.org/onto/class/google_cloudfunctions2_function"/>
    <rdfs:range rdf:resource="http://www.w3.org/2001/XMLSchema#string"/>
  </owl:DatatypeProperty>
  <owl:DatatypeProperty rdf:about="http://example.org/onto/prop/google_cloudfunctions2_function_retry_policy">
    <rdfs:label>retry_policy</rdfs:label>
    <rdfs:comment>Describes the retry policy in case of function's execution failure.
Retried execution is charged as any other execution. Possible values: ["RETRY_POLICY_UNSPECIFIED", "RETRY_POLICY_DO_NOT_RETRY", "RETRY_POLICY_RETRY"]</rdfs:comment>
    <rdfs:domain rdf:resource="http://example.org/onto/class/google_cloudfunctions2_function"/>
    <rdfs:range rdf:resource="http://www.w3.org/2001/XMLSchema#string"/>
  </owl:DatatypeProperty>
  <owl:DatatypeProperty rdf:about="http://example.org/onto/prop/google_cloudfunctions2_function_service_account_email">
    <rdfs:label>service_account_email</rdfs:label>
    <rdfs:comment>Optional. The email of the trigger's service account. The service account
must have permission to invoke Cloud Run services. If empty, defaults to the
Compute Engine default service account: {project_number}-compute@developer.gserviceaccount.com.</rdfs:comment>
    <rdfs:domain rdf:resource="http://example.org/onto/class/google_cloudfunctions2_function"/>
    <rdfs:range rdf:resource="http://www.w3.org/2001/XMLSchema#string"/>
  </owl:DatatypeProperty>
  <owl:DatatypeProperty rdf:about="http://example.org/onto/prop/google_cloudfunctions2_function_trigger">
    <rdfs:label>trigger</rdfs:label>
    <rdfs:comment>Output only. The resource name of the Eventarc trigger.</rdfs:comment>
    <rdfs:domain rdf:resource="http://example.org/onto/class/google_cloudfunctions2_function"/>
    <rdfs:range rdf:resource="http://www.w3.org/2001/XMLSchema#string"/>
  </owl:DatatypeProperty>
  <owl:DatatypeProperty rdf:about="http://example.org/onto/prop/google_cloudfunctions2_function_trigger_region">
    <rdfs:label>trigger_region</rdfs:label>
    <rdfs:comment>The region that the trigger will be in. The trigger will only receive
events originating in this region. It can be the same
region as the function, a different region or multi-region, or the global
region. If not provided, defaults to the same region as the function.</rdfs:comment>
    <rdfs:domain rdf:resource="http://example.org/onto/class/google_cloudfunctions2_function"/>
    <rdfs:range rdf:resource="http://www.w3.org/2001/XMLSchema#string"/>
  </owl:DatatypeProperty>
  <owl:DatatypeProperty rdf:about="http://example.org/onto/prop/google_cloudfunctions2_function_attribute">
    <rdfs:label>attribute</rdfs:label>
    <rdfs:comment>'Required. The name of a CloudEvents attribute.
Currently, only a subset of attributes are supported for filtering. Use the 'gcloud eventarc providers describe' command to learn more about events and their attributes.
Do not filter for the 'type' attribute here, as this is already achieved by the resource's 'event_type' attribute.</rdfs:comment>
    <rdfs:domain rdf:resource="http://example.org/onto/class/google_cloudfunctions2_function"/>
    <rdfs:range rdf:resource="http://www.w3.org/2001/XMLSchema#string"/>
  </owl:DatatypeProperty>
  <owl:DatatypeProperty rdf:about="http://example.org/onto/prop/google_cloudfunctions2_function_operator">
    <rdfs:label>operator</rdfs:label>
    <rdfs:comment>Optional. The operator used for matching the events with the value of
the filter. If not specified, only events that have an exact key-value
pair specified in the filter are matched.
The only allowed value is 'match-path-pattern'.
[See documentation on path patterns here](https://cloud.google.com/eventarc/docs/path-patterns)'</rdfs:comment>
    <rdfs:domain rdf:resource="http://example.org/onto/class/google_cloudfunctions2_function"/>
    <rdfs:range rdf:resource="http://www.w3.org/2001/XMLSchema#string"/>
  </owl:DatatypeProperty>
  <owl:DatatypeProperty rdf:about="http://example.org/onto/prop/google_cloudfunctions2_function_value">
    <rdfs:label>value</rdfs:label>
    <rdfs:comment>Required. The value for the attribute.
If the operator field is set as 'match-path-pattern', this value can be a path pattern instead of an exact value.</rdfs:comment>
    <rdfs:domain rdf:resource="http://example.org/onto/class/google_cloudfunctions2_function"/>
    <rdfs:range rdf:resource="http://www.w3.org/2001/XMLSchema#string"/>
  </owl:DatatypeProperty>
  <owl:DatatypeProperty rdf:about="http://example.org/onto/prop/google_cloudfunctions2_function_all_traffic_on_latest_revision">
    <rdfs:label>all_traffic_on_latest_revision</rdfs:label>
    <rdfs:comment>Whether 100% of traffic is routed to the latest revision. Defaults to true.</rdfs:comment>
    <rdfs:domain rdf:resource="http://example.org/onto/class/google_cloudfunctions2_function"/>
    <rdfs:range rdf:resource="http://www.w3.org/2001/XMLSchema#string"/>
  </owl:DatatypeProperty>
  <owl:DatatypeProperty rdf:about="http://example.org/onto/prop/google_cloudfunctions2_function_available_cpu">
    <rdfs:label>available_cpu</rdfs:label>
    <rdfs:comment>The number of CPUs used in a single container instance. Default value is calculated from available memory.</rdfs:comment>
    <rdfs:domain rdf:resource="http://example.org/onto/class/google_cloudfunctions2_function"/>
    <rdfs:range rdf:resource="http://www.w3.org/2001/XMLSchema#string"/>
  </owl:DatatypeProperty>
  <owl:DatatypeProperty rdf:about="http://example.org/onto/prop/google_cloudfunctions2_function_available_memory">
    <rdfs:label>available_memory</rdfs:label>
    <rdfs:comment>The amount of memory available for a function.
Defaults to 256M. Supported units are k, M, G, Mi, Gi. If no unit is
supplied the value is interpreted as bytes.</rdfs:comment>
    <rdfs:domain rdf:resource="http://example.org/onto/class/google_cloudfunctions2_function"/>
    <rdfs:range rdf:resource="http://www.w3.org/2001/XMLSchema#string"/>
  </owl:DatatypeProperty>
  <owl:DatatypeProperty rdf:about="http://example.org/onto/prop/google_cloudfunctions2_function_binary_authorization_policy">
    <rdfs:label>binary_authorization_policy</rdfs:label>
    <rdfs:comment>The binary authorization policy to be checked when deploying the Cloud Run service.</rdfs:comment>
    <rdfs:domain rdf:resource="http://example.org/onto/class/google_cloudfunctions2_function"/>
    <rdfs:range rdf:resource="http://www.w3.org/2001/XMLSchema#string"/>
  </owl:DatatypeProperty>
  <owl:DatatypeProperty rdf:about="http://example.org/onto/prop/google_cloudfunctions2_function_environment_variables">
    <rdfs:label>environment_variables</rdfs:label>
    <rdfs:comment>Environment variables that shall be available during function execution.</rdfs:comment>
    <rdfs:domain rdf:resource="http://example.org/onto/class/google_cloudfunctions2_function"/>
    <rdfs:range rdf:resource="http://www.w3.org/2001/XMLSchema#string"/>
  </owl:DatatypeProperty>
  <owl:DatatypeProperty rdf:about="http://example.org/onto/prop/google_cloudfunctions2_function_gcf_uri">
    <rdfs:label>gcf_uri</rdfs:label>
    <rdfs:comment>URIs of the Service deployed</rdfs:comment>
    <rdfs:domain rdf:resource="http://example.org/onto/class/google_cloudfunctions2_function"/>
    <rdfs:range rdf:resource="http://www.w3.org/2001/XMLSchema#string"/>
  </owl:DatatypeProperty>
  <owl:DatatypeProperty rdf:about="http://example.org/onto/prop/google_cloudfunctions2_function_ingress_settings">
    <rdfs:label>ingress_settings</rdfs:label>
    <rdfs:comment>Available ingress settings. Defaults to "ALLOW_ALL" if unspecified. Default value: "ALLOW_ALL" Possible values: ["ALLOW_ALL", "ALLOW_INTERNAL_ONLY", "ALLOW_INTERNAL_AND_GCLB"]</rdfs:comment>
    <rdfs:domain rdf:resource="http://example.org/onto/class/google_cloudfunctions2_function"/>
    <rdfs:range rdf:resource="http://www.w3.org/2001/XMLSchema#string"/>
  </owl:DatatypeProperty>
  <owl:DatatypeProperty rdf:about="http://example.org/onto/prop/google_cloudfunctions2_function_max_instance_count">
    <rdfs:label>max_instance_count</rdfs:label>
    <rdfs:comment>The limit on the maximum number of function instances that may coexist at a
given time.</rdfs:comment>
    <rdfs:domain rdf:resource="http://example.org/onto/class/google_cloudfunctions2_function"/>
    <rdfs:range rdf:resource="http://www.w3.org/2001/XMLSchema#string"/>
  </owl:DatatypeProperty>
  <owl:DatatypeProperty rdf:about="http://example.org/onto/prop/google_cloudfunctions2_function_max_instance_request_concurrency">
    <rdfs:label>max_instance_request_concurrency</rdfs:label>
    <rdfs:comment>Sets the maximum number of concurrent requests that each instance can receive. Defaults to 1.</rdfs:comment>
    <rdfs:domain rdf:resource="http://example.org/onto/class/google_cloudfunctions2_function"/>
    <rdfs:range rdf:resource="http://www.w3.org/2001/XMLSchema#string"/>
  </owl:DatatypeProperty>
  <owl:DatatypeProperty rdf:about="http://example.org/onto/prop/google_cloudfunctions2_function_min_instance_count">
    <rdfs:label>min_instance_count</rdfs:label>
    <rdfs:comment>The limit on the minimum number of function instances that may coexist at a
given time.</rdfs:comment>
    <rdfs:domain rdf:resource="http://example.org/onto/class/google_cloudfunctions2_function"/>
    <rdfs:range rdf:resource="http://www.w3.org/2001/XMLSchema#string"/>
  </owl:DatatypeProperty>
  <owl:DatatypeProperty rdf:about="http://example.org/onto/prop/google_cloudfunctions2_function_service">
    <rdfs:label>service</rdfs:label>
    <rdfs:comment>Name of the service associated with a Function.</rdfs:comment>
    <rdfs:domain rdf:resource="http://example.org/onto/class/google_cloudfunctions2_function"/>
    <rdfs:range rdf:resource="http://www.w3.org/2001/XMLSchema#string"/>
  </owl:DatatypeProperty>
  <owl:DatatypeProperty rdf:about="http://example.org/onto/prop/google_cloudfunctions2_function_service_account_email">
    <rdfs:label>service_account_email</rdfs:label>
    <rdfs:comment>The email of the service account for this function.</rdfs:comment>
    <rdfs:domain rdf:resource="http://example.org/onto/class/google_cloudfunctions2_function"/>
    <rdfs:range rdf:resource="http://www.w3.org/2001/XMLSchema#string"/>
  </owl:DatatypeProperty>
  <owl:DatatypeProperty rdf:about="http://example.org/onto/prop/google_cloudfunctions2_function_timeout_seconds">
    <rdfs:label>timeout_seconds</rdfs:label>
    <rdfs:comment>The function execution timeout. Execution is considered failed and
can be terminated if the function is not completed at the end of the
timeout period. Defaults to 60 seconds.</rdfs:comment>
    <rdfs:domain rdf:resource="http://example.org/onto/class/google_cloudfunctions2_function"/>
    <rdfs:range rdf:resource="http://www.w3.org/2001/XMLSchema#string"/>
  </owl:DatatypeProperty>
  <owl:DatatypeProperty rdf:about="http://example.org/onto/prop/google_cloudfunctions2_function_uri">
    <rdfs:label>uri</rdfs:label>
    <rdfs:comment>URI of the Service deployed.</rdfs:comment>
    <rdfs:domain rdf:resource="http://example.org/onto/class/google_cloudfunctions2_function"/>
    <rdfs:range rdf:resource="http://www.w3.org/2001/XMLSchema#string"/>
  </owl:DatatypeProperty>
  <owl:DatatypeProperty rdf:about="http://example.org/onto/prop/google_cloudfunctions2_function_vpc_connector">
    <rdfs:label>vpc_connector</rdfs:label>
    <rdfs:comment>The Serverless VPC Access connector that this cloud function can connect to.</rdfs:comment>
    <rdfs:domain rdf:resource="http://example.org/onto/class/google_cloudfunctions2_function"/>
    <rdfs:range rdf:resource="http://www.w3.org/2001/XMLSchema#string"/>
  </owl:DatatypeProperty>
  <owl:DatatypeProperty rdf:about="http://example.org/onto/prop/google_cloudfunctions2_function_vpc_connector_egress_settings">
    <rdfs:label>vpc_connector_egress_settings</rdfs:label>
    <rdfs:comment>Available egress settings. Possible values: ["VPC_CONNECTOR_EGRESS_SETTINGS_UNSPECIFIED", "PRIVATE_RANGES_ONLY", "ALL_TRAFFIC"]</rdfs:comment>
    <rdfs:domain rdf:resource="http://example.org/onto/class/google_cloudfunctions2_function"/>
    <rdfs:range rdf:resource="http://www.w3.org/2001/XMLSchema#string"/>
  </owl:DatatypeProperty>
  <owl:DatatypeProperty rdf:about="http://example.org/onto/prop/google_cloudfunctions2_function_key">
    <rdfs:label>key</rdfs:label>
    <rdfs:comment>Name of the environment variable.</rdfs:comment>
    <rdfs:domain rdf:resource="http://example.org/onto/class/google_cloudfunctions2_function"/>
    <rdfs:range rdf:resource="http://www.w3.org/2001/XMLSchema#string"/>
  </owl:DatatypeProperty>
  <owl:DatatypeProperty rdf:about="http://example.org/onto/prop/google_cloudfunctions2_function_project_id">
    <rdfs:label>project_id</rdfs:label>
    <rdfs:comment>Project identifier (preferably project number but can also be the project ID) of the project that contains the secret. If not set, it will be populated with the function's project assuming that the secret exists in the same project as of the function.</rdfs:comment>
    <rdfs:domain rdf:resource="http://example.org/onto/class/google_cloudfunctions2_function"/>
    <rdfs:range rdf:resource="http://www.w3.org/2001/XMLSchema#string"/>
  </owl:DatatypeProperty>
  <owl:DatatypeProperty rdf:about="http://example.org/onto/prop/google_cloudfunctions2_function_secret">
    <rdfs:label>secret</rdfs:label>
    <rdfs:comment>Name of the secret in secret manager (not the full resource name).</rdfs:comment>
    <rdfs:domain rdf:resource="http://example.org/onto/class/google_cloudfunctions2_function"/>
    <rdfs:range rdf:resource="http://www.w3.org/2001/XMLSchema#string"/>
  </owl:DatatypeProperty>
  <owl:DatatypeProperty rdf:about="http://example.org/onto/prop/google_cloudfunctions2_function_version">
    <rdfs:label>version</rdfs:label>
    <rdfs:comment>Version of the secret (version number or the string 'latest'). It is recommended to use a numeric version for secret environment variables as any updates to the secret value is not reflected until new instances start.</rdfs:comment>
    <rdfs:domain rdf:resource="http://example.org/onto/class/google_cloudfunctions2_function"/>
    <rdfs:range rdf:resource="http://www.w3.org/2001/XMLSchema#string"/>
  </owl:DatatypeProperty>
  <owl:DatatypeProperty rdf:about="http://example.org/onto/prop/google_cloudfunctions2_function_mount_path">
    <rdfs:label>mount_path</rdfs:label>
    <rdfs:comment>The path within the container to mount the secret volume. For example, setting the mountPath as /etc/secrets would mount the secret value files under the /etc/secrets directory. This directory will also be completely shadowed and unavailable to mount any other secrets. Recommended mount path: /etc/secrets</rdfs:comment>
    <rdfs:domain rdf:resource="http://example.org/onto/class/google_cloudfunctions2_function"/>
    <rdfs:range rdf:resource="http://www.w3.org/2001/XMLSchema#string"/>
  </owl:DatatypeProperty>
  <owl:DatatypeProperty rdf:about="http://example.org/onto/prop/google_cloudfunctions2_function_project_id">
    <rdfs:label>project_id</rdfs:label>
    <rdfs:comment>Project identifier (preferably project number but can also be the project ID) of the project that contains the secret. If not set, it will be populated with the function's project assuming that the secret exists in the same project as of the function.</rdfs:comment>
    <rdfs:domain rdf:resource="http://example.org/onto/class/google_cloudfunctions2_function"/>
    <rdfs:range rdf:resource="http://www.w3.org/2001/XMLSchema#string"/>
  </owl:DatatypeProperty>
  <owl:DatatypeProperty rdf:about="http://example.org/onto/prop/google_cloudfunctions2_function_secret">
    <rdfs:label>secret</rdfs:label>
    <rdfs:comment>Name of the secret in secret manager (not the full resource name).</rdfs:comment>
    <rdfs:domain rdf:resource="http://example.org/onto/class/google_cloudfunctions2_function"/>
    <rdfs:range rdf:resource="http://www.w3.org/2001/XMLSchema#string"/>
  </owl:DatatypeProperty>
  <owl:DatatypeProperty rdf:about="http://example.org/onto/prop/google_cloudfunctions2_function_path">
    <rdfs:label>path</rdfs:label>
    <rdfs:comment>Relative path of the file under the mount path where the secret value for this version will be fetched and made available. For example, setting the mountPath as '/etc/secrets' and path as secret_foo would mount the secret value file at /etc/secrets/secret_foo.</rdfs:comment>
    <rdfs:domain rdf:resource="http://example.org/onto/class/google_cloudfunctions2_function"/>
    <rdfs:range rdf:resource="http://www.w3.org/2001/XMLSchema#string"/>
  </owl:DatatypeProperty>
  <owl:DatatypeProperty rdf:about="http://example.org/onto/prop/google_cloudfunctions2_function_version">
    <rdfs:label>version</rdfs:label>
    <rdfs:comment>Version of the secret (version number or the string 'latest'). It is preferable to use latest version with secret volumes as secret value changes are reflected immediately.</rdfs:comment>
    <rdfs:domain rdf:resource="http://example.org/onto/class/google_cloudfunctions2_function"/>
    <rdfs:range rdf:resource="http://www.w3.org/2001/XMLSchema#string"/>
  </owl:DatatypeProperty>
  <owl:DatatypeProperty rdf:about="http://example.org/onto/prop/google_cloudfunctions2_function_create">
    <rdfs:label>create</rdfs:label>
    <rdfs:domain rdf:resource="http://example.org/onto/class/google_cloudfunctions2_function"/>
    <rdfs:range rdf:resource="http://www.w3.org/2001/XMLSchema#string"/>
  </owl:DatatypeProperty>
  <owl:DatatypeProperty rdf:about="http://example.org/onto/prop/google_cloudfunctions2_function_delete">
    <rdfs:label>delete</rdfs:label>
    <rdfs:domain rdf:resource="http://example.org/onto/class/google_cloudfunctions2_function"/>
    <rdfs:range rdf:resource="http://www.w3.org/2001/XMLSchema#string"/>
  </owl:DatatypeProperty>
  <owl:DatatypeProperty rdf:about="http://example.org/onto/prop/google_cloudfunctions2_function_update">
    <rdfs:label>update</rdfs:label>
    <rdfs:domain rdf:resource="http://example.org/onto/class/google_cloudfunctions2_function"/>
    <rdfs:range rdf:resource="http://www.w3.org/2001/XMLSchema#string"/>
  </owl:DatatypeProperty>
</rdf:RDF>
