<?xml version="1.0" encoding="UTF-8"?>
<rdf:RDF
  xmlns:rdf="http://www.w3.org/1999/02/22-rdf-syntax-ns#"
  xmlns:rdfs="http://www.w3.org/2000/01/rdf-schema#"
  xmlns:owl="http://www.w3.org/2002/07/owl#"
  xmlns:xsd="http://www.w3.org/2001/XMLSchema#"
  xml:base="http://example.org/onto/">
  <owl:Class rdf:about="http://example.org/onto/class/google_container_analysis_occurrence">
    <rdfs:label>google_container_analysis_occurrence</rdfs:label>
    <rdfs:comment>#
#     ***     AUTO GENERATED CODE    ***    Type: MMv1     ***
#
# ----------------------------------------------------------------------------
#
#     This code is generated by Magic Modules using the following:
#
#     Configuration: https:#github.com/GoogleCloudPlatform/magic-modules/tree/main/mmv1/products/containeranalysis/Occurrence.yaml
#     Template:      https:#github.com/GoogleCloudPlatform/magic-modules/tree/main/mmv1/templates/terraform/resource.html.markdown.tmpl
#
#     DO NOT EDIT this file directly. Any changes made to this file will be
#     overwritten during the next generation cycle.
#
# ----------------------------------------------------------------------------
subcategory: "Container Registry"
description: |-
  An occurrence is an instance of a Note, or type of analysis that
  can be done for a resource.
---</rdfs:comment>
  </owl:Class>
  <owl:DatatypeProperty rdf:about="http://example.org/onto/prop/google_container_analysis_occurrence_create_time">
    <rdfs:label>create_time</rdfs:label>
    <rdfs:comment>The time when the repository was created.</rdfs:comment>
    <rdfs:domain rdf:resource="http://example.org/onto/class/google_container_analysis_occurrence"/>
    <rdfs:range rdf:resource="http://www.w3.org/2001/XMLSchema#string"/>
  </owl:DatatypeProperty>
  <owl:DatatypeProperty rdf:about="http://example.org/onto/prop/google_container_analysis_occurrence_id">
    <rdfs:label>id</rdfs:label>
    <rdfs:domain rdf:resource="http://example.org/onto/class/google_container_analysis_occurrence"/>
    <rdfs:range rdf:resource="http://www.w3.org/2001/XMLSchema#string"/>
  </owl:DatatypeProperty>
  <owl:DatatypeProperty rdf:about="http://example.org/onto/prop/google_container_analysis_occurrence_kind">
    <rdfs:label>kind</rdfs:label>
    <rdfs:comment>The note kind which explicitly denotes which of the occurrence
details are specified. This field can be used as a filter in list
requests.</rdfs:comment>
    <rdfs:domain rdf:resource="http://example.org/onto/class/google_container_analysis_occurrence"/>
    <rdfs:range rdf:resource="http://www.w3.org/2001/XMLSchema#string"/>
  </owl:DatatypeProperty>
  <owl:DatatypeProperty rdf:about="http://example.org/onto/prop/google_container_analysis_occurrence_name">
    <rdfs:label>name</rdfs:label>
    <rdfs:comment>The name of the occurrence.</rdfs:comment>
    <rdfs:domain rdf:resource="http://example.org/onto/class/google_container_analysis_occurrence"/>
    <rdfs:range rdf:resource="http://www.w3.org/2001/XMLSchema#string"/>
  </owl:DatatypeProperty>
  <owl:DatatypeProperty rdf:about="http://example.org/onto/prop/google_container_analysis_occurrence_note_name">
    <rdfs:label>note_name</rdfs:label>
    <rdfs:comment>The analysis note associated with this occurrence, in the form of
projects/[PROJECT]/notes/[NOTE_ID]. This field can be used as a
filter in list requests.</rdfs:comment>
    <rdfs:domain rdf:resource="http://example.org/onto/class/google_container_analysis_occurrence"/>
    <rdfs:range rdf:resource="http://www.w3.org/2001/XMLSchema#string"/>
  </owl:DatatypeProperty>
  <owl:DatatypeProperty rdf:about="http://example.org/onto/prop/google_container_analysis_occurrence_project">
    <rdfs:label>project</rdfs:label>
    <rdfs:domain rdf:resource="http://example.org/onto/class/google_container_analysis_occurrence"/>
    <rdfs:range rdf:resource="http://www.w3.org/2001/XMLSchema#string"/>
  </owl:DatatypeProperty>
  <owl:DatatypeProperty rdf:about="http://example.org/onto/prop/google_container_analysis_occurrence_remediation">
    <rdfs:label>remediation</rdfs:label>
    <rdfs:comment>A description of actions that can be taken to remedy the note.</rdfs:comment>
    <rdfs:domain rdf:resource="http://example.org/onto/class/google_container_analysis_occurrence"/>
    <rdfs:range rdf:resource="http://www.w3.org/2001/XMLSchema#string"/>
  </owl:DatatypeProperty>
  <owl:DatatypeProperty rdf:about="http://example.org/onto/prop/google_container_analysis_occurrence_resource_uri">
    <rdfs:label>resource_uri</rdfs:label>
    <rdfs:comment>Required. Immutable. A URI that represents the resource for which
the occurrence applies. For example,
https://gcr.io/project/image@sha256:123abc for a Docker image.</rdfs:comment>
    <rdfs:domain rdf:resource="http://example.org/onto/class/google_container_analysis_occurrence"/>
    <rdfs:range rdf:resource="http://www.w3.org/2001/XMLSchema#string"/>
  </owl:DatatypeProperty>
  <owl:DatatypeProperty rdf:about="http://example.org/onto/prop/google_container_analysis_occurrence_update_time">
    <rdfs:label>update_time</rdfs:label>
    <rdfs:comment>The time when the repository was last updated.</rdfs:comment>
    <rdfs:domain rdf:resource="http://example.org/onto/class/google_container_analysis_occurrence"/>
    <rdfs:range rdf:resource="http://www.w3.org/2001/XMLSchema#string"/>
  </owl:DatatypeProperty>
  <owl:DatatypeProperty rdf:about="http://example.org/onto/prop/google_container_analysis_occurrence_serialized_payload">
    <rdfs:label>serialized_payload</rdfs:label>
    <rdfs:comment>The serialized payload that is verified by one or
more signatures. A base64-encoded string.</rdfs:comment>
    <rdfs:domain rdf:resource="http://example.org/onto/class/google_container_analysis_occurrence"/>
    <rdfs:range rdf:resource="http://www.w3.org/2001/XMLSchema#string"/>
  </owl:DatatypeProperty>
  <owl:DatatypeProperty rdf:about="http://example.org/onto/prop/google_container_analysis_occurrence_public_key_id">
    <rdfs:label>public_key_id</rdfs:label>
    <rdfs:comment>The identifier for the public key that verifies this
signature. MUST be an RFC3986 conformant
URI. * When possible, the key id should be an
immutable reference, such as a cryptographic digest.
Examples of valid values:

* OpenPGP V4 public key fingerprint. See https://www.iana.org/assignments/uri-schemes/prov/openpgp4fpr
  for more details on this scheme.
    * 'openpgp4fpr:74FAF3B861BDA0870C7B6DEF607E48D2A663AEEA'
* RFC6920 digest-named SubjectPublicKeyInfo (digest of the DER serialization):
    * "ni:///sha-256;cD9o9Cq6LG3jD0iKXqEi_vdjJGecm_iXkbqVoScViaU"</rdfs:comment>
    <rdfs:domain rdf:resource="http://example.org/onto/class/google_container_analysis_occurrence"/>
    <rdfs:range rdf:resource="http://www.w3.org/2001/XMLSchema#string"/>
  </owl:DatatypeProperty>
  <owl:DatatypeProperty rdf:about="http://example.org/onto/prop/google_container_analysis_occurrence_signature">
    <rdfs:label>signature</rdfs:label>
    <rdfs:comment>The content of the signature, an opaque bytestring.
The payload that this signature verifies MUST be
unambiguously provided with the Signature during
verification. A wrapper message might provide the
payload explicitly. Alternatively, a message might
have a canonical serialization that can always be
unambiguously computed to derive the payload.</rdfs:comment>
    <rdfs:domain rdf:resource="http://example.org/onto/class/google_container_analysis_occurrence"/>
    <rdfs:range rdf:resource="http://www.w3.org/2001/XMLSchema#string"/>
  </owl:DatatypeProperty>
  <owl:DatatypeProperty rdf:about="http://example.org/onto/prop/google_container_analysis_occurrence_create">
    <rdfs:label>create</rdfs:label>
    <rdfs:domain rdf:resource="http://example.org/onto/class/google_container_analysis_occurrence"/>
    <rdfs:range rdf:resource="http://www.w3.org/2001/XMLSchema#string"/>
  </owl:DatatypeProperty>
  <owl:DatatypeProperty rdf:about="http://example.org/onto/prop/google_container_analysis_occurrence_delete">
    <rdfs:label>delete</rdfs:label>
    <rdfs:domain rdf:resource="http://example.org/onto/class/google_container_analysis_occurrence"/>
    <rdfs:range rdf:resource="http://www.w3.org/2001/XMLSchema#string"/>
  </owl:DatatypeProperty>
  <owl:DatatypeProperty rdf:about="http://example.org/onto/prop/google_container_analysis_occurrence_update">
    <rdfs:label>update</rdfs:label>
    <rdfs:domain rdf:resource="http://example.org/onto/class/google_container_analysis_occurrence"/>
    <rdfs:range rdf:resource="http://www.w3.org/2001/XMLSchema#string"/>
  </owl:DatatypeProperty>
</rdf:RDF>
