<?xml version="1.0" encoding="UTF-8"?>
<rdf:RDF
  xmlns:rdf="http://www.w3.org/1999/02/22-rdf-syntax-ns#"
  xmlns:rdfs="http://www.w3.org/2000/01/rdf-schema#"
  xmlns:owl="http://www.w3.org/2002/07/owl#"
  xmlns:xsd="http://www.w3.org/2001/XMLSchema#"
  xml:base="http://example.org/onto/">
  <owl:Class rdf:about="http://example.org/onto/class/google_vertex_ai_featurestore_entitytype">
    <rdfs:label>google_vertex_ai_featurestore_entitytype</rdfs:label>
    <rdfs:comment>#
#     ***     AUTO GENERATED CODE    ***    Type: MMv1     ***
#
# ----------------------------------------------------------------------------
#
#     This code is generated by Magic Modules using the following:
#
#     Configuration: https:#github.com/GoogleCloudPlatform/magic-modules/tree/main/mmv1/products/vertexai/FeaturestoreEntitytype.yaml
#     Template:      https:#github.com/GoogleCloudPlatform/magic-modules/tree/main/mmv1/templates/terraform/resource.html.markdown.tmpl
#
#     DO NOT EDIT this file directly. Any changes made to this file will be
#     overwritten during the next generation cycle.
#
# ----------------------------------------------------------------------------
subcategory: "Vertex AI"
description: |-
  An entity type is a type of object in a system that needs to be modeled and have stored information about.
---</rdfs:comment>
  </owl:Class>
  <owl:DatatypeProperty rdf:about="http://example.org/onto/prop/google_vertex_ai_featurestore_entitytype_create_time">
    <rdfs:label>create_time</rdfs:label>
    <rdfs:comment>The timestamp of when the featurestore was created in RFC3339 UTC "Zulu" format, with nanosecond resolution and up to nine fractional digits.</rdfs:comment>
    <rdfs:domain rdf:resource="http://example.org/onto/class/google_vertex_ai_featurestore_entitytype"/>
    <rdfs:range rdf:resource="http://www.w3.org/2001/XMLSchema#string"/>
  </owl:DatatypeProperty>
  <owl:DatatypeProperty rdf:about="http://example.org/onto/prop/google_vertex_ai_featurestore_entitytype_description">
    <rdfs:label>description</rdfs:label>
    <rdfs:comment>Optional. Description of the EntityType.</rdfs:comment>
    <rdfs:domain rdf:resource="http://example.org/onto/class/google_vertex_ai_featurestore_entitytype"/>
    <rdfs:range rdf:resource="http://www.w3.org/2001/XMLSchema#string"/>
  </owl:DatatypeProperty>
  <owl:DatatypeProperty rdf:about="http://example.org/onto/prop/google_vertex_ai_featurestore_entitytype_effective_labels">
    <rdfs:label>effective_labels</rdfs:label>
    <rdfs:comment>All of labels (key/value pairs) present on the resource in GCP, including the labels configured through Terraform, other clients and services.</rdfs:comment>
    <rdfs:domain rdf:resource="http://example.org/onto/class/google_vertex_ai_featurestore_entitytype"/>
    <rdfs:range rdf:resource="http://www.w3.org/2001/XMLSchema#string"/>
  </owl:DatatypeProperty>
  <owl:DatatypeProperty rdf:about="http://example.org/onto/prop/google_vertex_ai_featurestore_entitytype_etag">
    <rdfs:label>etag</rdfs:label>
    <rdfs:comment>Used to perform consistent read-modify-write updates.</rdfs:comment>
    <rdfs:domain rdf:resource="http://example.org/onto/class/google_vertex_ai_featurestore_entitytype"/>
    <rdfs:range rdf:resource="http://www.w3.org/2001/XMLSchema#string"/>
  </owl:DatatypeProperty>
  <owl:DatatypeProperty rdf:about="http://example.org/onto/prop/google_vertex_ai_featurestore_entitytype_featurestore">
    <rdfs:label>featurestore</rdfs:label>
    <rdfs:comment>The name of the Featurestore to use, in the format projects/{project}/locations/{location}/featurestores/{featurestore}.</rdfs:comment>
    <rdfs:domain rdf:resource="http://example.org/onto/class/google_vertex_ai_featurestore_entitytype"/>
    <rdfs:range rdf:resource="http://www.w3.org/2001/XMLSchema#string"/>
  </owl:DatatypeProperty>
  <owl:DatatypeProperty rdf:about="http://example.org/onto/prop/google_vertex_ai_featurestore_entitytype_id">
    <rdfs:label>id</rdfs:label>
    <rdfs:domain rdf:resource="http://example.org/onto/class/google_vertex_ai_featurestore_entitytype"/>
    <rdfs:range rdf:resource="http://www.w3.org/2001/XMLSchema#string"/>
  </owl:DatatypeProperty>
  <owl:DatatypeProperty rdf:about="http://example.org/onto/prop/google_vertex_ai_featurestore_entitytype_labels">
    <rdfs:label>labels</rdfs:label>
    <rdfs:comment>A set of key/value label pairs to assign to this EntityType.


**Note**: This field is non-authoritative, and will only manage the labels present in your configuration.
Please refer to the field 'effective_labels' for all of the labels present on the resource.</rdfs:comment>
    <rdfs:domain rdf:resource="http://example.org/onto/class/google_vertex_ai_featurestore_entitytype"/>
    <rdfs:range rdf:resource="http://www.w3.org/2001/XMLSchema#string"/>
  </owl:DatatypeProperty>
  <owl:DatatypeProperty rdf:about="http://example.org/onto/prop/google_vertex_ai_featurestore_entitytype_name">
    <rdfs:label>name</rdfs:label>
    <rdfs:comment>The name of the EntityType. This value may be up to 60 characters, and valid characters are [a-z0-9_]. The first character cannot be a number.</rdfs:comment>
    <rdfs:domain rdf:resource="http://example.org/onto/class/google_vertex_ai_featurestore_entitytype"/>
    <rdfs:range rdf:resource="http://www.w3.org/2001/XMLSchema#string"/>
  </owl:DatatypeProperty>
  <owl:DatatypeProperty rdf:about="http://example.org/onto/prop/google_vertex_ai_featurestore_entitytype_region">
    <rdfs:label>region</rdfs:label>
    <rdfs:comment>The region of the EntityType.</rdfs:comment>
    <rdfs:domain rdf:resource="http://example.org/onto/class/google_vertex_ai_featurestore_entitytype"/>
    <rdfs:range rdf:resource="http://www.w3.org/2001/XMLSchema#string"/>
  </owl:DatatypeProperty>
  <owl:DatatypeProperty rdf:about="http://example.org/onto/prop/google_vertex_ai_featurestore_entitytype_terraform_labels">
    <rdfs:label>terraform_labels</rdfs:label>
    <rdfs:comment>The combination of labels configured directly on the resource
 and default labels configured on the provider.</rdfs:comment>
    <rdfs:domain rdf:resource="http://example.org/onto/class/google_vertex_ai_featurestore_entitytype"/>
    <rdfs:range rdf:resource="http://www.w3.org/2001/XMLSchema#string"/>
  </owl:DatatypeProperty>
  <owl:DatatypeProperty rdf:about="http://example.org/onto/prop/google_vertex_ai_featurestore_entitytype_update_time">
    <rdfs:label>update_time</rdfs:label>
    <rdfs:comment>The timestamp of when the featurestore was last updated in RFC3339 UTC "Zulu" format, with nanosecond resolution and up to nine fractional digits.</rdfs:comment>
    <rdfs:domain rdf:resource="http://example.org/onto/class/google_vertex_ai_featurestore_entitytype"/>
    <rdfs:range rdf:resource="http://www.w3.org/2001/XMLSchema#string"/>
  </owl:DatatypeProperty>
  <owl:DatatypeProperty rdf:about="http://example.org/onto/prop/google_vertex_ai_featurestore_entitytype_value">
    <rdfs:label>value</rdfs:label>
    <rdfs:comment>Specify a threshold value that can trigger the alert. For categorical feature, the distribution distance is calculated by L-inifinity norm. Each feature must have a non-zero threshold if they need to be monitored. Otherwise no alert will be triggered for that feature. The default value is 0.3.</rdfs:comment>
    <rdfs:domain rdf:resource="http://example.org/onto/class/google_vertex_ai_featurestore_entitytype"/>
    <rdfs:range rdf:resource="http://www.w3.org/2001/XMLSchema#string"/>
  </owl:DatatypeProperty>
  <owl:DatatypeProperty rdf:about="http://example.org/onto/prop/google_vertex_ai_featurestore_entitytype_anomaly_detection_baseline">
    <rdfs:label>anomaly_detection_baseline</rdfs:label>
    <rdfs:comment>Defines the baseline to do anomaly detection for feature values imported by each [entityTypes.importFeatureValues][] operation. The value must be one of the values below:
* LATEST_STATS: Choose the later one statistics generated by either most recent snapshot analysis or previous import features analysis. If non of them exists, skip anomaly detection and only generate a statistics.
* MOST_RECENT_SNAPSHOT_STATS: Use the statistics generated by the most recent snapshot analysis if exists.
* PREVIOUS_IMPORT_FEATURES_STATS: Use the statistics generated by the previous import features analysis if exists.</rdfs:comment>
    <rdfs:domain rdf:resource="http://example.org/onto/class/google_vertex_ai_featurestore_entitytype"/>
    <rdfs:range rdf:resource="http://www.w3.org/2001/XMLSchema#string"/>
  </owl:DatatypeProperty>
  <owl:DatatypeProperty rdf:about="http://example.org/onto/prop/google_vertex_ai_featurestore_entitytype_state">
    <rdfs:label>state</rdfs:label>
    <rdfs:comment>Whether to enable / disable / inherite default hebavior for import features analysis. The value must be one of the values below:
* DEFAULT: The default behavior of whether to enable the monitoring. EntityType-level config: disabled.
* ENABLED: Explicitly enables import features analysis. EntityType-level config: by default enables import features analysis for all Features under it.
* DISABLED: Explicitly disables import features analysis. EntityType-level config: by default disables import features analysis for all Features under it.</rdfs:comment>
    <rdfs:domain rdf:resource="http://example.org/onto/class/google_vertex_ai_featurestore_entitytype"/>
    <rdfs:range rdf:resource="http://www.w3.org/2001/XMLSchema#string"/>
  </owl:DatatypeProperty>
  <owl:DatatypeProperty rdf:about="http://example.org/onto/prop/google_vertex_ai_featurestore_entitytype_value">
    <rdfs:label>value</rdfs:label>
    <rdfs:comment>Specify a threshold value that can trigger the alert. For numerical feature, the distribution distance is calculated by Jensenâ€“Shannon divergence. Each feature must have a non-zero threshold if they need to be monitored. Otherwise no alert will be triggered for that feature. The default value is 0.3.</rdfs:comment>
    <rdfs:domain rdf:resource="http://example.org/onto/class/google_vertex_ai_featurestore_entitytype"/>
    <rdfs:range rdf:resource="http://www.w3.org/2001/XMLSchema#string"/>
  </owl:DatatypeProperty>
  <owl:DatatypeProperty rdf:about="http://example.org/onto/prop/google_vertex_ai_featurestore_entitytype_disabled">
    <rdfs:label>disabled</rdfs:label>
    <rdfs:comment>The monitoring schedule for snapshot analysis. For EntityType-level config: unset / disabled = true indicates disabled by default for Features under it; otherwise by default enable snapshot analysis monitoring with monitoringInterval for Features under it.</rdfs:comment>
    <rdfs:domain rdf:resource="http://example.org/onto/class/google_vertex_ai_featurestore_entitytype"/>
    <rdfs:range rdf:resource="http://www.w3.org/2001/XMLSchema#string"/>
  </owl:DatatypeProperty>
  <owl:DatatypeProperty rdf:about="http://example.org/onto/prop/google_vertex_ai_featurestore_entitytype_monitoring_interval_days">
    <rdfs:label>monitoring_interval_days</rdfs:label>
    <rdfs:comment>Configuration of the snapshot analysis based monitoring pipeline running interval. The value indicates number of days. The default value is 1.
If both FeaturestoreMonitoringConfig.SnapshotAnalysis.monitoring_interval_days and [FeaturestoreMonitoringConfig.SnapshotAnalysis.monitoring_interval][] are set when creating/updating EntityTypes/Features, FeaturestoreMonitoringConfig.SnapshotAnalysis.monitoring_interval_days will be used.</rdfs:comment>
    <rdfs:domain rdf:resource="http://example.org/onto/class/google_vertex_ai_featurestore_entitytype"/>
    <rdfs:range rdf:resource="http://www.w3.org/2001/XMLSchema#string"/>
  </owl:DatatypeProperty>
  <owl:DatatypeProperty rdf:about="http://example.org/onto/prop/google_vertex_ai_featurestore_entitytype_staleness_days">
    <rdfs:label>staleness_days</rdfs:label>
    <rdfs:comment>Customized export features time window for snapshot analysis. Unit is one day. The default value is 21 days. Minimum value is 1 day. Maximum value is 4000 days.</rdfs:comment>
    <rdfs:domain rdf:resource="http://example.org/onto/class/google_vertex_ai_featurestore_entitytype"/>
    <rdfs:range rdf:resource="http://www.w3.org/2001/XMLSchema#string"/>
  </owl:DatatypeProperty>
  <owl:DatatypeProperty rdf:about="http://example.org/onto/prop/google_vertex_ai_featurestore_entitytype_create">
    <rdfs:label>create</rdfs:label>
    <rdfs:domain rdf:resource="http://example.org/onto/class/google_vertex_ai_featurestore_entitytype"/>
    <rdfs:range rdf:resource="http://www.w3.org/2001/XMLSchema#string"/>
  </owl:DatatypeProperty>
  <owl:DatatypeProperty rdf:about="http://example.org/onto/prop/google_vertex_ai_featurestore_entitytype_delete">
    <rdfs:label>delete</rdfs:label>
    <rdfs:domain rdf:resource="http://example.org/onto/class/google_vertex_ai_featurestore_entitytype"/>
    <rdfs:range rdf:resource="http://www.w3.org/2001/XMLSchema#string"/>
  </owl:DatatypeProperty>
  <owl:DatatypeProperty rdf:about="http://example.org/onto/prop/google_vertex_ai_featurestore_entitytype_update">
    <rdfs:label>update</rdfs:label>
    <rdfs:domain rdf:resource="http://example.org/onto/class/google_vertex_ai_featurestore_entitytype"/>
    <rdfs:range rdf:resource="http://www.w3.org/2001/XMLSchema#string"/>
  </owl:DatatypeProperty>
</rdf:RDF>
