<?xml version="1.0" encoding="UTF-8"?>
<rdf:RDF
  xmlns:rdf="http://www.w3.org/1999/02/22-rdf-syntax-ns#"
  xmlns:rdfs="http://www.w3.org/2000/01/rdf-schema#"
  xmlns:owl="http://www.w3.org/2002/07/owl#"
  xmlns:xsd="http://www.w3.org/2001/XMLSchema#"
  xml:base="http://example.org/onto/">
  <owl:Class rdf:about="http://example.org/onto/class/google_compute_region_health_check">
    <rdfs:label>google_compute_region_health_check</rdfs:label>
    <rdfs:comment>#
#     ***     AUTO GENERATED CODE    ***    Type: MMv1     ***
#
# ----------------------------------------------------------------------------
#
#     This code is generated by Magic Modules using the following:
#
#     Configuration: https:#github.com/GoogleCloudPlatform/magic-modules/tree/main/mmv1/products/compute/RegionHealthCheck.yaml
#     Template:      https:#github.com/GoogleCloudPlatform/magic-modules/tree/main/mmv1/templates/terraform/resource.html.markdown.tmpl
#
#     DO NOT EDIT this file directly. Any changes made to this file will be
#     overwritten during the next generation cycle.
#
# ----------------------------------------------------------------------------
subcategory: "Compute Engine"
description: |-
  Health Checks determine whether instances are responsive and able to do work.
---</rdfs:comment>
  </owl:Class>
  <owl:DatatypeProperty rdf:about="http://example.org/onto/prop/google_compute_region_health_check_check_interval_sec">
    <rdfs:label>check_interval_sec</rdfs:label>
    <rdfs:comment>How often (in seconds) to send a health check. The default value is 5
seconds.</rdfs:comment>
    <rdfs:domain rdf:resource="http://example.org/onto/class/google_compute_region_health_check"/>
    <rdfs:range rdf:resource="http://www.w3.org/2001/XMLSchema#string"/>
  </owl:DatatypeProperty>
  <owl:DatatypeProperty rdf:about="http://example.org/onto/prop/google_compute_region_health_check_creation_timestamp">
    <rdfs:label>creation_timestamp</rdfs:label>
    <rdfs:comment>Creation timestamp in RFC3339 text format.</rdfs:comment>
    <rdfs:domain rdf:resource="http://example.org/onto/class/google_compute_region_health_check"/>
    <rdfs:range rdf:resource="http://www.w3.org/2001/XMLSchema#string"/>
  </owl:DatatypeProperty>
  <owl:DatatypeProperty rdf:about="http://example.org/onto/prop/google_compute_region_health_check_description">
    <rdfs:label>description</rdfs:label>
    <rdfs:comment>An optional description of this resource. Provide this property when
you create the resource.</rdfs:comment>
    <rdfs:domain rdf:resource="http://example.org/onto/class/google_compute_region_health_check"/>
    <rdfs:range rdf:resource="http://www.w3.org/2001/XMLSchema#string"/>
  </owl:DatatypeProperty>
  <owl:DatatypeProperty rdf:about="http://example.org/onto/prop/google_compute_region_health_check_health_check_id">
    <rdfs:label>health_check_id</rdfs:label>
    <rdfs:comment>The unique identifier number for the resource. This identifier is defined by the server.</rdfs:comment>
    <rdfs:domain rdf:resource="http://example.org/onto/class/google_compute_region_health_check"/>
    <rdfs:range rdf:resource="http://www.w3.org/2001/XMLSchema#string"/>
  </owl:DatatypeProperty>
  <owl:DatatypeProperty rdf:about="http://example.org/onto/prop/google_compute_region_health_check_healthy_threshold">
    <rdfs:label>healthy_threshold</rdfs:label>
    <rdfs:comment>A so-far unhealthy instance will be marked healthy after this many
consecutive successes. The default value is 2.</rdfs:comment>
    <rdfs:domain rdf:resource="http://example.org/onto/class/google_compute_region_health_check"/>
    <rdfs:range rdf:resource="http://www.w3.org/2001/XMLSchema#string"/>
  </owl:DatatypeProperty>
  <owl:DatatypeProperty rdf:about="http://example.org/onto/prop/google_compute_region_health_check_id">
    <rdfs:label>id</rdfs:label>
    <rdfs:domain rdf:resource="http://example.org/onto/class/google_compute_region_health_check"/>
    <rdfs:range rdf:resource="http://www.w3.org/2001/XMLSchema#string"/>
  </owl:DatatypeProperty>
  <owl:DatatypeProperty rdf:about="http://example.org/onto/prop/google_compute_region_health_check_name">
    <rdfs:label>name</rdfs:label>
    <rdfs:comment>Name of the resource. Provided by the client when the resource is
created. The name must be 1-63 characters long, and comply with
RFC1035.  Specifically, the name must be 1-63 characters long and
match the regular expression '[a-z]([-a-z0-9]*[a-z0-9])?' which means
the first character must be a lowercase letter, and all following
characters must be a dash, lowercase letter, or digit, except the
last character, which cannot be a dash.</rdfs:comment>
    <rdfs:domain rdf:resource="http://example.org/onto/class/google_compute_region_health_check"/>
    <rdfs:range rdf:resource="http://www.w3.org/2001/XMLSchema#string"/>
  </owl:DatatypeProperty>
  <owl:DatatypeProperty rdf:about="http://example.org/onto/prop/google_compute_region_health_check_project">
    <rdfs:label>project</rdfs:label>
    <rdfs:domain rdf:resource="http://example.org/onto/class/google_compute_region_health_check"/>
    <rdfs:range rdf:resource="http://www.w3.org/2001/XMLSchema#string"/>
  </owl:DatatypeProperty>
  <owl:DatatypeProperty rdf:about="http://example.org/onto/prop/google_compute_region_health_check_region">
    <rdfs:label>region</rdfs:label>
    <rdfs:comment>The Region in which the created health check should reside.
If it is not provided, the provider region is used.</rdfs:comment>
    <rdfs:domain rdf:resource="http://example.org/onto/class/google_compute_region_health_check"/>
    <rdfs:range rdf:resource="http://www.w3.org/2001/XMLSchema#string"/>
  </owl:DatatypeProperty>
  <owl:DatatypeProperty rdf:about="http://example.org/onto/prop/google_compute_region_health_check_self_link">
    <rdfs:label>self_link</rdfs:label>
    <rdfs:domain rdf:resource="http://example.org/onto/class/google_compute_region_health_check"/>
    <rdfs:range rdf:resource="http://www.w3.org/2001/XMLSchema#string"/>
  </owl:DatatypeProperty>
  <owl:DatatypeProperty rdf:about="http://example.org/onto/prop/google_compute_region_health_check_timeout_sec">
    <rdfs:label>timeout_sec</rdfs:label>
    <rdfs:comment>How long (in seconds) to wait before claiming failure.
The default value is 5 seconds.  It is invalid for timeoutSec to have
greater value than checkIntervalSec.</rdfs:comment>
    <rdfs:domain rdf:resource="http://example.org/onto/class/google_compute_region_health_check"/>
    <rdfs:range rdf:resource="http://www.w3.org/2001/XMLSchema#string"/>
  </owl:DatatypeProperty>
  <owl:DatatypeProperty rdf:about="http://example.org/onto/prop/google_compute_region_health_check_type">
    <rdfs:label>type</rdfs:label>
    <rdfs:comment>The type of the health check. One of HTTP, HTTP2, HTTPS, TCP, or SSL.</rdfs:comment>
    <rdfs:domain rdf:resource="http://example.org/onto/class/google_compute_region_health_check"/>
    <rdfs:range rdf:resource="http://www.w3.org/2001/XMLSchema#string"/>
  </owl:DatatypeProperty>
  <owl:DatatypeProperty rdf:about="http://example.org/onto/prop/google_compute_region_health_check_unhealthy_threshold">
    <rdfs:label>unhealthy_threshold</rdfs:label>
    <rdfs:comment>A so-far healthy instance will be marked unhealthy after this many
consecutive failures. The default value is 2.</rdfs:comment>
    <rdfs:domain rdf:resource="http://example.org/onto/class/google_compute_region_health_check"/>
    <rdfs:range rdf:resource="http://www.w3.org/2001/XMLSchema#string"/>
  </owl:DatatypeProperty>
  <owl:DatatypeProperty rdf:about="http://example.org/onto/prop/google_compute_region_health_check_grpc_service_name">
    <rdfs:label>grpc_service_name</rdfs:label>
    <rdfs:comment>The gRPC service name for the health check.
The value of grpcServiceName has the following meanings by convention:

* Empty serviceName means the overall status of all services at the backend.
* Non-empty serviceName means the health of that gRPC service, as defined by the owner of the service.

The grpcServiceName can only be ASCII.</rdfs:comment>
    <rdfs:domain rdf:resource="http://example.org/onto/class/google_compute_region_health_check"/>
    <rdfs:range rdf:resource="http://www.w3.org/2001/XMLSchema#string"/>
  </owl:DatatypeProperty>
  <owl:DatatypeProperty rdf:about="http://example.org/onto/prop/google_compute_region_health_check_port">
    <rdfs:label>port</rdfs:label>
    <rdfs:comment>The port number for the health check request.
Must be specified if portName and portSpecification are not set
or if port_specification is USE_FIXED_PORT. Valid values are 1 through 65535.</rdfs:comment>
    <rdfs:domain rdf:resource="http://example.org/onto/class/google_compute_region_health_check"/>
    <rdfs:range rdf:resource="http://www.w3.org/2001/XMLSchema#string"/>
  </owl:DatatypeProperty>
  <owl:DatatypeProperty rdf:about="http://example.org/onto/prop/google_compute_region_health_check_port_name">
    <rdfs:label>port_name</rdfs:label>
    <rdfs:comment>Port name as defined in InstanceGroup#NamedPort#name. If both port and
port_name are defined, port takes precedence.</rdfs:comment>
    <rdfs:domain rdf:resource="http://example.org/onto/class/google_compute_region_health_check"/>
    <rdfs:range rdf:resource="http://www.w3.org/2001/XMLSchema#string"/>
  </owl:DatatypeProperty>
  <owl:DatatypeProperty rdf:about="http://example.org/onto/prop/google_compute_region_health_check_port_specification">
    <rdfs:label>port_specification</rdfs:label>
    <rdfs:comment>Specifies how port is selected for health checking, can be one of the
following values:

  * 'USE_FIXED_PORT': The port number in 'port' is used for health checking.

  * 'USE_NAMED_PORT': The 'portName' is used for health checking.

  * 'USE_SERVING_PORT': For NetworkEndpointGroup, the port specified for each
  network endpoint is used for health checking. For other backends, the
  port or named port specified in the Backend Service is used for health
  checking.

If not specified, gRPC health check follows behavior specified in 'port' and
'portName' fields. Possible values: ["USE_FIXED_PORT", "USE_NAMED_PORT", "USE_SERVING_PORT"]</rdfs:comment>
    <rdfs:domain rdf:resource="http://example.org/onto/class/google_compute_region_health_check"/>
    <rdfs:range rdf:resource="http://www.w3.org/2001/XMLSchema#string"/>
  </owl:DatatypeProperty>
  <owl:DatatypeProperty rdf:about="http://example.org/onto/prop/google_compute_region_health_check_host">
    <rdfs:label>host</rdfs:label>
    <rdfs:comment>The value of the host header in the HTTP2 health check request.
If left empty (default value), the public IP on behalf of which this health
check is performed will be used.</rdfs:comment>
    <rdfs:domain rdf:resource="http://example.org/onto/class/google_compute_region_health_check"/>
    <rdfs:range rdf:resource="http://www.w3.org/2001/XMLSchema#string"/>
  </owl:DatatypeProperty>
  <owl:DatatypeProperty rdf:about="http://example.org/onto/prop/google_compute_region_health_check_port">
    <rdfs:label>port</rdfs:label>
    <rdfs:comment>The TCP port number for the HTTP2 health check request.
The default value is 443.</rdfs:comment>
    <rdfs:domain rdf:resource="http://example.org/onto/class/google_compute_region_health_check"/>
    <rdfs:range rdf:resource="http://www.w3.org/2001/XMLSchema#string"/>
  </owl:DatatypeProperty>
  <owl:DatatypeProperty rdf:about="http://example.org/onto/prop/google_compute_region_health_check_port_name">
    <rdfs:label>port_name</rdfs:label>
    <rdfs:comment>Port name as defined in InstanceGroup#NamedPort#name. If both port and
port_name are defined, port takes precedence.</rdfs:comment>
    <rdfs:domain rdf:resource="http://example.org/onto/class/google_compute_region_health_check"/>
    <rdfs:range rdf:resource="http://www.w3.org/2001/XMLSchema#string"/>
  </owl:DatatypeProperty>
  <owl:DatatypeProperty rdf:about="http://example.org/onto/prop/google_compute_region_health_check_port_specification">
    <rdfs:label>port_specification</rdfs:label>
    <rdfs:comment>Specifies how port is selected for health checking, can be one of the
following values:

  * 'USE_FIXED_PORT': The port number in 'port' is used for health checking.

  * 'USE_NAMED_PORT': The 'portName' is used for health checking.

  * 'USE_SERVING_PORT': For NetworkEndpointGroup, the port specified for each
  network endpoint is used for health checking. For other backends, the
  port or named port specified in the Backend Service is used for health
  checking.

If not specified, HTTP2 health check follows behavior specified in 'port' and
'portName' fields. Possible values: ["USE_FIXED_PORT", "USE_NAMED_PORT", "USE_SERVING_PORT"]</rdfs:comment>
    <rdfs:domain rdf:resource="http://example.org/onto/class/google_compute_region_health_check"/>
    <rdfs:range rdf:resource="http://www.w3.org/2001/XMLSchema#string"/>
  </owl:DatatypeProperty>
  <owl:DatatypeProperty rdf:about="http://example.org/onto/prop/google_compute_region_health_check_proxy_header">
    <rdfs:label>proxy_header</rdfs:label>
    <rdfs:comment>Specifies the type of proxy header to append before sending data to the
backend. Default value: "NONE" Possible values: ["NONE", "PROXY_V1"]</rdfs:comment>
    <rdfs:domain rdf:resource="http://example.org/onto/class/google_compute_region_health_check"/>
    <rdfs:range rdf:resource="http://www.w3.org/2001/XMLSchema#string"/>
  </owl:DatatypeProperty>
  <owl:DatatypeProperty rdf:about="http://example.org/onto/prop/google_compute_region_health_check_request_path">
    <rdfs:label>request_path</rdfs:label>
    <rdfs:comment>The request path of the HTTP2 health check request.
The default value is /.</rdfs:comment>
    <rdfs:domain rdf:resource="http://example.org/onto/class/google_compute_region_health_check"/>
    <rdfs:range rdf:resource="http://www.w3.org/2001/XMLSchema#string"/>
  </owl:DatatypeProperty>
  <owl:DatatypeProperty rdf:about="http://example.org/onto/prop/google_compute_region_health_check_response">
    <rdfs:label>response</rdfs:label>
    <rdfs:comment>The bytes to match against the beginning of the response data. If left empty
(the default value), any response will indicate health. The response data
can only be ASCII.</rdfs:comment>
    <rdfs:domain rdf:resource="http://example.org/onto/class/google_compute_region_health_check"/>
    <rdfs:range rdf:resource="http://www.w3.org/2001/XMLSchema#string"/>
  </owl:DatatypeProperty>
  <owl:DatatypeProperty rdf:about="http://example.org/onto/prop/google_compute_region_health_check_host">
    <rdfs:label>host</rdfs:label>
    <rdfs:comment>The value of the host header in the HTTP health check request.
If left empty (default value), the public IP on behalf of which this health
check is performed will be used.</rdfs:comment>
    <rdfs:domain rdf:resource="http://example.org/onto/class/google_compute_region_health_check"/>
    <rdfs:range rdf:resource="http://www.w3.org/2001/XMLSchema#string"/>
  </owl:DatatypeProperty>
  <owl:DatatypeProperty rdf:about="http://example.org/onto/prop/google_compute_region_health_check_port">
    <rdfs:label>port</rdfs:label>
    <rdfs:comment>The TCP port number for the HTTP health check request.
The default value is 80.</rdfs:comment>
    <rdfs:domain rdf:resource="http://example.org/onto/class/google_compute_region_health_check"/>
    <rdfs:range rdf:resource="http://www.w3.org/2001/XMLSchema#string"/>
  </owl:DatatypeProperty>
  <owl:DatatypeProperty rdf:about="http://example.org/onto/prop/google_compute_region_health_check_port_name">
    <rdfs:label>port_name</rdfs:label>
    <rdfs:comment>Port name as defined in InstanceGroup#NamedPort#name. If both port and
port_name are defined, port takes precedence.</rdfs:comment>
    <rdfs:domain rdf:resource="http://example.org/onto/class/google_compute_region_health_check"/>
    <rdfs:range rdf:resource="http://www.w3.org/2001/XMLSchema#string"/>
  </owl:DatatypeProperty>
  <owl:DatatypeProperty rdf:about="http://example.org/onto/prop/google_compute_region_health_check_port_specification">
    <rdfs:label>port_specification</rdfs:label>
    <rdfs:comment>Specifies how port is selected for health checking, can be one of the
following values:

  * 'USE_FIXED_PORT': The port number in 'port' is used for health checking.

  * 'USE_NAMED_PORT': The 'portName' is used for health checking.

  * 'USE_SERVING_PORT': For NetworkEndpointGroup, the port specified for each
  network endpoint is used for health checking. For other backends, the
  port or named port specified in the Backend Service is used for health
  checking.

If not specified, HTTP health check follows behavior specified in 'port' and
'portName' fields. Possible values: ["USE_FIXED_PORT", "USE_NAMED_PORT", "USE_SERVING_PORT"]</rdfs:comment>
    <rdfs:domain rdf:resource="http://example.org/onto/class/google_compute_region_health_check"/>
    <rdfs:range rdf:resource="http://www.w3.org/2001/XMLSchema#string"/>
  </owl:DatatypeProperty>
  <owl:DatatypeProperty rdf:about="http://example.org/onto/prop/google_compute_region_health_check_proxy_header">
    <rdfs:label>proxy_header</rdfs:label>
    <rdfs:comment>Specifies the type of proxy header to append before sending data to the
backend. Default value: "NONE" Possible values: ["NONE", "PROXY_V1"]</rdfs:comment>
    <rdfs:domain rdf:resource="http://example.org/onto/class/google_compute_region_health_check"/>
    <rdfs:range rdf:resource="http://www.w3.org/2001/XMLSchema#string"/>
  </owl:DatatypeProperty>
  <owl:DatatypeProperty rdf:about="http://example.org/onto/prop/google_compute_region_health_check_request_path">
    <rdfs:label>request_path</rdfs:label>
    <rdfs:comment>The request path of the HTTP health check request.
The default value is /.</rdfs:comment>
    <rdfs:domain rdf:resource="http://example.org/onto/class/google_compute_region_health_check"/>
    <rdfs:range rdf:resource="http://www.w3.org/2001/XMLSchema#string"/>
  </owl:DatatypeProperty>
  <owl:DatatypeProperty rdf:about="http://example.org/onto/prop/google_compute_region_health_check_response">
    <rdfs:label>response</rdfs:label>
    <rdfs:comment>The bytes to match against the beginning of the response data. If left empty
(the default value), any response will indicate health. The response data
can only be ASCII.</rdfs:comment>
    <rdfs:domain rdf:resource="http://example.org/onto/class/google_compute_region_health_check"/>
    <rdfs:range rdf:resource="http://www.w3.org/2001/XMLSchema#string"/>
  </owl:DatatypeProperty>
  <owl:DatatypeProperty rdf:about="http://example.org/onto/prop/google_compute_region_health_check_host">
    <rdfs:label>host</rdfs:label>
    <rdfs:comment>The value of the host header in the HTTPS health check request.
If left empty (default value), the public IP on behalf of which this health
check is performed will be used.</rdfs:comment>
    <rdfs:domain rdf:resource="http://example.org/onto/class/google_compute_region_health_check"/>
    <rdfs:range rdf:resource="http://www.w3.org/2001/XMLSchema#string"/>
  </owl:DatatypeProperty>
  <owl:DatatypeProperty rdf:about="http://example.org/onto/prop/google_compute_region_health_check_port">
    <rdfs:label>port</rdfs:label>
    <rdfs:comment>The TCP port number for the HTTPS health check request.
The default value is 443.</rdfs:comment>
    <rdfs:domain rdf:resource="http://example.org/onto/class/google_compute_region_health_check"/>
    <rdfs:range rdf:resource="http://www.w3.org/2001/XMLSchema#string"/>
  </owl:DatatypeProperty>
  <owl:DatatypeProperty rdf:about="http://example.org/onto/prop/google_compute_region_health_check_port_name">
    <rdfs:label>port_name</rdfs:label>
    <rdfs:comment>Port name as defined in InstanceGroup#NamedPort#name. If both port and
port_name are defined, port takes precedence.</rdfs:comment>
    <rdfs:domain rdf:resource="http://example.org/onto/class/google_compute_region_health_check"/>
    <rdfs:range rdf:resource="http://www.w3.org/2001/XMLSchema#string"/>
  </owl:DatatypeProperty>
  <owl:DatatypeProperty rdf:about="http://example.org/onto/prop/google_compute_region_health_check_port_specification">
    <rdfs:label>port_specification</rdfs:label>
    <rdfs:comment>Specifies how port is selected for health checking, can be one of the
following values:

  * 'USE_FIXED_PORT': The port number in 'port' is used for health checking.

  * 'USE_NAMED_PORT': The 'portName' is used for health checking.

  * 'USE_SERVING_PORT': For NetworkEndpointGroup, the port specified for each
  network endpoint is used for health checking. For other backends, the
  port or named port specified in the Backend Service is used for health
  checking.

If not specified, HTTPS health check follows behavior specified in 'port' and
'portName' fields. Possible values: ["USE_FIXED_PORT", "USE_NAMED_PORT", "USE_SERVING_PORT"]</rdfs:comment>
    <rdfs:domain rdf:resource="http://example.org/onto/class/google_compute_region_health_check"/>
    <rdfs:range rdf:resource="http://www.w3.org/2001/XMLSchema#string"/>
  </owl:DatatypeProperty>
  <owl:DatatypeProperty rdf:about="http://example.org/onto/prop/google_compute_region_health_check_proxy_header">
    <rdfs:label>proxy_header</rdfs:label>
    <rdfs:comment>Specifies the type of proxy header to append before sending data to the
backend. Default value: "NONE" Possible values: ["NONE", "PROXY_V1"]</rdfs:comment>
    <rdfs:domain rdf:resource="http://example.org/onto/class/google_compute_region_health_check"/>
    <rdfs:range rdf:resource="http://www.w3.org/2001/XMLSchema#string"/>
  </owl:DatatypeProperty>
  <owl:DatatypeProperty rdf:about="http://example.org/onto/prop/google_compute_region_health_check_request_path">
    <rdfs:label>request_path</rdfs:label>
    <rdfs:comment>The request path of the HTTPS health check request.
The default value is /.</rdfs:comment>
    <rdfs:domain rdf:resource="http://example.org/onto/class/google_compute_region_health_check"/>
    <rdfs:range rdf:resource="http://www.w3.org/2001/XMLSchema#string"/>
  </owl:DatatypeProperty>
  <owl:DatatypeProperty rdf:about="http://example.org/onto/prop/google_compute_region_health_check_response">
    <rdfs:label>response</rdfs:label>
    <rdfs:comment>The bytes to match against the beginning of the response data. If left empty
(the default value), any response will indicate health. The response data
can only be ASCII.</rdfs:comment>
    <rdfs:domain rdf:resource="http://example.org/onto/class/google_compute_region_health_check"/>
    <rdfs:range rdf:resource="http://www.w3.org/2001/XMLSchema#string"/>
  </owl:DatatypeProperty>
  <owl:DatatypeProperty rdf:about="http://example.org/onto/prop/google_compute_region_health_check_enable">
    <rdfs:label>enable</rdfs:label>
    <rdfs:comment>Indicates whether or not to export logs. This is false by default,
which means no health check logging will be done.</rdfs:comment>
    <rdfs:domain rdf:resource="http://example.org/onto/class/google_compute_region_health_check"/>
    <rdfs:range rdf:resource="http://www.w3.org/2001/XMLSchema#string"/>
  </owl:DatatypeProperty>
  <owl:DatatypeProperty rdf:about="http://example.org/onto/prop/google_compute_region_health_check_port">
    <rdfs:label>port</rdfs:label>
    <rdfs:comment>The TCP port number for the SSL health check request.
The default value is 443.</rdfs:comment>
    <rdfs:domain rdf:resource="http://example.org/onto/class/google_compute_region_health_check"/>
    <rdfs:range rdf:resource="http://www.w3.org/2001/XMLSchema#string"/>
  </owl:DatatypeProperty>
  <owl:DatatypeProperty rdf:about="http://example.org/onto/prop/google_compute_region_health_check_port_name">
    <rdfs:label>port_name</rdfs:label>
    <rdfs:comment>Port name as defined in InstanceGroup#NamedPort#name. If both port and
port_name are defined, port takes precedence.</rdfs:comment>
    <rdfs:domain rdf:resource="http://example.org/onto/class/google_compute_region_health_check"/>
    <rdfs:range rdf:resource="http://www.w3.org/2001/XMLSchema#string"/>
  </owl:DatatypeProperty>
  <owl:DatatypeProperty rdf:about="http://example.org/onto/prop/google_compute_region_health_check_port_specification">
    <rdfs:label>port_specification</rdfs:label>
    <rdfs:comment>Specifies how port is selected for health checking, can be one of the
following values:

  * 'USE_FIXED_PORT': The port number in 'port' is used for health checking.

  * 'USE_NAMED_PORT': The 'portName' is used for health checking.

  * 'USE_SERVING_PORT': For NetworkEndpointGroup, the port specified for each
  network endpoint is used for health checking. For other backends, the
  port or named port specified in the Backend Service is used for health
  checking.

If not specified, SSL health check follows behavior specified in 'port' and
'portName' fields. Possible values: ["USE_FIXED_PORT", "USE_NAMED_PORT", "USE_SERVING_PORT"]</rdfs:comment>
    <rdfs:domain rdf:resource="http://example.org/onto/class/google_compute_region_health_check"/>
    <rdfs:range rdf:resource="http://www.w3.org/2001/XMLSchema#string"/>
  </owl:DatatypeProperty>
  <owl:DatatypeProperty rdf:about="http://example.org/onto/prop/google_compute_region_health_check_proxy_header">
    <rdfs:label>proxy_header</rdfs:label>
    <rdfs:comment>Specifies the type of proxy header to append before sending data to the
backend. Default value: "NONE" Possible values: ["NONE", "PROXY_V1"]</rdfs:comment>
    <rdfs:domain rdf:resource="http://example.org/onto/class/google_compute_region_health_check"/>
    <rdfs:range rdf:resource="http://www.w3.org/2001/XMLSchema#string"/>
  </owl:DatatypeProperty>
  <owl:DatatypeProperty rdf:about="http://example.org/onto/prop/google_compute_region_health_check_request">
    <rdfs:label>request</rdfs:label>
    <rdfs:comment>The application data to send once the SSL connection has been
established (default value is empty). If both request and response are
empty, the connection establishment alone will indicate health. The request
data can only be ASCII.</rdfs:comment>
    <rdfs:domain rdf:resource="http://example.org/onto/class/google_compute_region_health_check"/>
    <rdfs:range rdf:resource="http://www.w3.org/2001/XMLSchema#string"/>
  </owl:DatatypeProperty>
  <owl:DatatypeProperty rdf:about="http://example.org/onto/prop/google_compute_region_health_check_response">
    <rdfs:label>response</rdfs:label>
    <rdfs:comment>The bytes to match against the beginning of the response data. If left empty
(the default value), any response will indicate health. The response data
can only be ASCII.</rdfs:comment>
    <rdfs:domain rdf:resource="http://example.org/onto/class/google_compute_region_health_check"/>
    <rdfs:range rdf:resource="http://www.w3.org/2001/XMLSchema#string"/>
  </owl:DatatypeProperty>
  <owl:DatatypeProperty rdf:about="http://example.org/onto/prop/google_compute_region_health_check_port">
    <rdfs:label>port</rdfs:label>
    <rdfs:comment>The TCP port number for the TCP health check request.
The default value is 80.</rdfs:comment>
    <rdfs:domain rdf:resource="http://example.org/onto/class/google_compute_region_health_check"/>
    <rdfs:range rdf:resource="http://www.w3.org/2001/XMLSchema#string"/>
  </owl:DatatypeProperty>
  <owl:DatatypeProperty rdf:about="http://example.org/onto/prop/google_compute_region_health_check_port_name">
    <rdfs:label>port_name</rdfs:label>
    <rdfs:comment>Port name as defined in InstanceGroup#NamedPort#name. If both port and
port_name are defined, port takes precedence.</rdfs:comment>
    <rdfs:domain rdf:resource="http://example.org/onto/class/google_compute_region_health_check"/>
    <rdfs:range rdf:resource="http://www.w3.org/2001/XMLSchema#string"/>
  </owl:DatatypeProperty>
  <owl:DatatypeProperty rdf:about="http://example.org/onto/prop/google_compute_region_health_check_port_specification">
    <rdfs:label>port_specification</rdfs:label>
    <rdfs:comment>Specifies how port is selected for health checking, can be one of the
following values:

  * 'USE_FIXED_PORT': The port number in 'port' is used for health checking.

  * 'USE_NAMED_PORT': The 'portName' is used for health checking.

  * 'USE_SERVING_PORT': For NetworkEndpointGroup, the port specified for each
  network endpoint is used for health checking. For other backends, the
  port or named port specified in the Backend Service is used for health
  checking.

If not specified, TCP health check follows behavior specified in 'port' and
'portName' fields. Possible values: ["USE_FIXED_PORT", "USE_NAMED_PORT", "USE_SERVING_PORT"]</rdfs:comment>
    <rdfs:domain rdf:resource="http://example.org/onto/class/google_compute_region_health_check"/>
    <rdfs:range rdf:resource="http://www.w3.org/2001/XMLSchema#string"/>
  </owl:DatatypeProperty>
  <owl:DatatypeProperty rdf:about="http://example.org/onto/prop/google_compute_region_health_check_proxy_header">
    <rdfs:label>proxy_header</rdfs:label>
    <rdfs:comment>Specifies the type of proxy header to append before sending data to the
backend. Default value: "NONE" Possible values: ["NONE", "PROXY_V1"]</rdfs:comment>
    <rdfs:domain rdf:resource="http://example.org/onto/class/google_compute_region_health_check"/>
    <rdfs:range rdf:resource="http://www.w3.org/2001/XMLSchema#string"/>
  </owl:DatatypeProperty>
  <owl:DatatypeProperty rdf:about="http://example.org/onto/prop/google_compute_region_health_check_request">
    <rdfs:label>request</rdfs:label>
    <rdfs:comment>The application data to send once the TCP connection has been
established (default value is empty). If both request and response are
empty, the connection establishment alone will indicate health. The request
data can only be ASCII.</rdfs:comment>
    <rdfs:domain rdf:resource="http://example.org/onto/class/google_compute_region_health_check"/>
    <rdfs:range rdf:resource="http://www.w3.org/2001/XMLSchema#string"/>
  </owl:DatatypeProperty>
  <owl:DatatypeProperty rdf:about="http://example.org/onto/prop/google_compute_region_health_check_response">
    <rdfs:label>response</rdfs:label>
    <rdfs:comment>The bytes to match against the beginning of the response data. If left empty
(the default value), any response will indicate health. The response data
can only be ASCII.</rdfs:comment>
    <rdfs:domain rdf:resource="http://example.org/onto/class/google_compute_region_health_check"/>
    <rdfs:range rdf:resource="http://www.w3.org/2001/XMLSchema#string"/>
  </owl:DatatypeProperty>
  <owl:DatatypeProperty rdf:about="http://example.org/onto/prop/google_compute_region_health_check_create">
    <rdfs:label>create</rdfs:label>
    <rdfs:domain rdf:resource="http://example.org/onto/class/google_compute_region_health_check"/>
    <rdfs:range rdf:resource="http://www.w3.org/2001/XMLSchema#string"/>
  </owl:DatatypeProperty>
  <owl:DatatypeProperty rdf:about="http://example.org/onto/prop/google_compute_region_health_check_delete">
    <rdfs:label>delete</rdfs:label>
    <rdfs:domain rdf:resource="http://example.org/onto/class/google_compute_region_health_check"/>
    <rdfs:range rdf:resource="http://www.w3.org/2001/XMLSchema#string"/>
  </owl:DatatypeProperty>
  <owl:DatatypeProperty rdf:about="http://example.org/onto/prop/google_compute_region_health_check_update">
    <rdfs:label>update</rdfs:label>
    <rdfs:domain rdf:resource="http://example.org/onto/class/google_compute_region_health_check"/>
    <rdfs:range rdf:resource="http://www.w3.org/2001/XMLSchema#string"/>
  </owl:DatatypeProperty>
</rdf:RDF>
