<?xml version="1.0" encoding="UTF-8"?>
<rdf:RDF
  xmlns:rdf="http://www.w3.org/1999/02/22-rdf-syntax-ns#"
  xmlns:rdfs="http://www.w3.org/2000/01/rdf-schema#"
  xmlns:owl="http://www.w3.org/2002/07/owl#"
  xmlns:xsd="http://www.w3.org/2001/XMLSchema#"
  xml:base="http://example.org/onto/">
  <owl:Class rdf:about="http://example.org/onto/class/google_monitoring_uptime_check_config">
    <rdfs:label>google_monitoring_uptime_check_config</rdfs:label>
    <rdfs:comment>#
#     ***     AUTO GENERATED CODE    ***    Type: MMv1     ***
#
# ----------------------------------------------------------------------------
#
#     This code is generated by Magic Modules using the following:
#
#     Configuration: https:#github.com/GoogleCloudPlatform/magic-modules/tree/main/mmv1/products/monitoring/UptimeCheckConfig.yaml
#     Template:      https:#github.com/GoogleCloudPlatform/magic-modules/tree/main/mmv1/templates/terraform/resource.html.markdown.tmpl
#
#     DO NOT EDIT this file directly. Any changes made to this file will be
#     overwritten during the next generation cycle.
#
# ----------------------------------------------------------------------------
subcategory: "Cloud (Stackdriver) Monitoring"
description: |-
  This message configures which resources and services to monitor for availability.
---</rdfs:comment>
  </owl:Class>
  <owl:DatatypeProperty rdf:about="http://example.org/onto/prop/google_monitoring_uptime_check_config_checker_type">
    <rdfs:label>checker_type</rdfs:label>
    <rdfs:comment>The checker type to use for the check. If the monitored resource type is 'servicedirectory_service', 'checker_type' must be set to 'VPC_CHECKERS'. Possible values: ["STATIC_IP_CHECKERS", "VPC_CHECKERS"]</rdfs:comment>
    <rdfs:domain rdf:resource="http://example.org/onto/class/google_monitoring_uptime_check_config"/>
    <rdfs:range rdf:resource="http://www.w3.org/2001/XMLSchema#string"/>
  </owl:DatatypeProperty>
  <owl:DatatypeProperty rdf:about="http://example.org/onto/prop/google_monitoring_uptime_check_config_display_name">
    <rdfs:label>display_name</rdfs:label>
    <rdfs:comment>A human-friendly name for the uptime check configuration. The display name should be unique within a Stackdriver Workspace in order to make it easier to identify; however, uniqueness is not enforced.</rdfs:comment>
    <rdfs:domain rdf:resource="http://example.org/onto/class/google_monitoring_uptime_check_config"/>
    <rdfs:range rdf:resource="http://www.w3.org/2001/XMLSchema#string"/>
  </owl:DatatypeProperty>
  <owl:DatatypeProperty rdf:about="http://example.org/onto/prop/google_monitoring_uptime_check_config_id">
    <rdfs:label>id</rdfs:label>
    <rdfs:domain rdf:resource="http://example.org/onto/class/google_monitoring_uptime_check_config"/>
    <rdfs:range rdf:resource="http://www.w3.org/2001/XMLSchema#string"/>
  </owl:DatatypeProperty>
  <owl:DatatypeProperty rdf:about="http://example.org/onto/prop/google_monitoring_uptime_check_config_log_check_failures">
    <rdfs:label>log_check_failures</rdfs:label>
    <rdfs:comment>Specifies whether to log the results of failed probes to Cloud Logging.</rdfs:comment>
    <rdfs:domain rdf:resource="http://example.org/onto/class/google_monitoring_uptime_check_config"/>
    <rdfs:range rdf:resource="http://www.w3.org/2001/XMLSchema#string"/>
  </owl:DatatypeProperty>
  <owl:DatatypeProperty rdf:about="http://example.org/onto/prop/google_monitoring_uptime_check_config_name">
    <rdfs:label>name</rdfs:label>
    <rdfs:comment>A unique resource name for this UptimeCheckConfig. The format is 'projects/[PROJECT_ID]/uptimeCheckConfigs/[UPTIME_CHECK_ID]'.</rdfs:comment>
    <rdfs:domain rdf:resource="http://example.org/onto/class/google_monitoring_uptime_check_config"/>
    <rdfs:range rdf:resource="http://www.w3.org/2001/XMLSchema#string"/>
  </owl:DatatypeProperty>
  <owl:DatatypeProperty rdf:about="http://example.org/onto/prop/google_monitoring_uptime_check_config_period">
    <rdfs:label>period</rdfs:label>
    <rdfs:comment>How often, in seconds, the uptime check is performed. Currently, the only supported values are 60s (1 minute), 300s (5 minutes), 600s (10 minutes), and 900s (15 minutes). Optional, defaults to 300s.</rdfs:comment>
    <rdfs:domain rdf:resource="http://example.org/onto/class/google_monitoring_uptime_check_config"/>
    <rdfs:range rdf:resource="http://www.w3.org/2001/XMLSchema#string"/>
  </owl:DatatypeProperty>
  <owl:DatatypeProperty rdf:about="http://example.org/onto/prop/google_monitoring_uptime_check_config_project">
    <rdfs:label>project</rdfs:label>
    <rdfs:domain rdf:resource="http://example.org/onto/class/google_monitoring_uptime_check_config"/>
    <rdfs:range rdf:resource="http://www.w3.org/2001/XMLSchema#string"/>
  </owl:DatatypeProperty>
  <owl:DatatypeProperty rdf:about="http://example.org/onto/prop/google_monitoring_uptime_check_config_selected_regions">
    <rdfs:label>selected_regions</rdfs:label>
    <rdfs:comment>The list of regions from which the check will be run. Some regions contain one location, and others contain more than one. If this field is specified, enough regions to include a minimum of 3 locations must be provided, or an error message is returned. Not specifying this field will result in uptime checks running from all regions.</rdfs:comment>
    <rdfs:domain rdf:resource="http://example.org/onto/class/google_monitoring_uptime_check_config"/>
    <rdfs:range rdf:resource="http://www.w3.org/2001/XMLSchema#string"/>
  </owl:DatatypeProperty>
  <owl:DatatypeProperty rdf:about="http://example.org/onto/prop/google_monitoring_uptime_check_config_timeout">
    <rdfs:label>timeout</rdfs:label>
    <rdfs:comment>The maximum amount of time to wait for the request to complete (must be between 1 and 60 seconds). [See the accepted formats]( https://developers.google.com/protocol-buffers/docs/reference/google.protobuf#google.protobuf.Duration)</rdfs:comment>
    <rdfs:domain rdf:resource="http://example.org/onto/class/google_monitoring_uptime_check_config"/>
    <rdfs:range rdf:resource="http://www.w3.org/2001/XMLSchema#string"/>
  </owl:DatatypeProperty>
  <owl:DatatypeProperty rdf:about="http://example.org/onto/prop/google_monitoring_uptime_check_config_uptime_check_id">
    <rdfs:label>uptime_check_id</rdfs:label>
    <rdfs:comment>The id of the uptime check</rdfs:comment>
    <rdfs:domain rdf:resource="http://example.org/onto/class/google_monitoring_uptime_check_config"/>
    <rdfs:range rdf:resource="http://www.w3.org/2001/XMLSchema#string"/>
  </owl:DatatypeProperty>
  <owl:DatatypeProperty rdf:about="http://example.org/onto/prop/google_monitoring_uptime_check_config_user_labels">
    <rdfs:label>user_labels</rdfs:label>
    <rdfs:comment>User-supplied key/value data to be used for organizing and identifying the 'UptimeCheckConfig' objects. The field can contain up to 64 entries. Each key and value is limited to 63 Unicode characters or 128 bytes, whichever is smaller. Labels and values can contain only lowercase letters, numerals, underscores, and dashes. Keys must begin with a letter.</rdfs:comment>
    <rdfs:domain rdf:resource="http://example.org/onto/class/google_monitoring_uptime_check_config"/>
    <rdfs:range rdf:resource="http://www.w3.org/2001/XMLSchema#string"/>
  </owl:DatatypeProperty>
  <owl:DatatypeProperty rdf:about="http://example.org/onto/prop/google_monitoring_uptime_check_config_content">
    <rdfs:label>content</rdfs:label>
    <rdfs:comment>String or regex content to match (max 1024 bytes)</rdfs:comment>
    <rdfs:domain rdf:resource="http://example.org/onto/class/google_monitoring_uptime_check_config"/>
    <rdfs:range rdf:resource="http://www.w3.org/2001/XMLSchema#string"/>
  </owl:DatatypeProperty>
  <owl:DatatypeProperty rdf:about="http://example.org/onto/prop/google_monitoring_uptime_check_config_matcher">
    <rdfs:label>matcher</rdfs:label>
    <rdfs:comment>The type of content matcher that will be applied to the server output, compared to the content string when the check is run. Default value: "CONTAINS_STRING" Possible values: ["CONTAINS_STRING", "NOT_CONTAINS_STRING", "MATCHES_REGEX", "NOT_MATCHES_REGEX", "MATCHES_JSON_PATH", "NOT_MATCHES_JSON_PATH"]</rdfs:comment>
    <rdfs:domain rdf:resource="http://example.org/onto/class/google_monitoring_uptime_check_config"/>
    <rdfs:range rdf:resource="http://www.w3.org/2001/XMLSchema#string"/>
  </owl:DatatypeProperty>
  <owl:DatatypeProperty rdf:about="http://example.org/onto/prop/google_monitoring_uptime_check_config_json_matcher">
    <rdfs:label>json_matcher</rdfs:label>
    <rdfs:comment>Options to perform JSONPath content matching. Default value: "EXACT_MATCH" Possible values: ["EXACT_MATCH", "REGEX_MATCH"]</rdfs:comment>
    <rdfs:domain rdf:resource="http://example.org/onto/class/google_monitoring_uptime_check_config"/>
    <rdfs:range rdf:resource="http://www.w3.org/2001/XMLSchema#string"/>
  </owl:DatatypeProperty>
  <owl:DatatypeProperty rdf:about="http://example.org/onto/prop/google_monitoring_uptime_check_config_json_path">
    <rdfs:label>json_path</rdfs:label>
    <rdfs:comment>JSONPath within the response output pointing to the expected 'ContentMatcher::content' to match against.</rdfs:comment>
    <rdfs:domain rdf:resource="http://example.org/onto/class/google_monitoring_uptime_check_config"/>
    <rdfs:range rdf:resource="http://www.w3.org/2001/XMLSchema#string"/>
  </owl:DatatypeProperty>
  <owl:DatatypeProperty rdf:about="http://example.org/onto/prop/google_monitoring_uptime_check_config_body">
    <rdfs:label>body</rdfs:label>
    <rdfs:comment>The request body associated with the HTTP POST request. If 'content_type' is 'URL_ENCODED', the body passed in must be URL-encoded. Users can provide a 'Content-Length' header via the 'headers' field or the API will do so. If the 'request_method' is 'GET' and 'body' is not empty, the API will return an error. The maximum byte size is 1 megabyte. Note - As with all bytes fields JSON representations are base64 encoded. e.g. 'foo=bar' in URL-encoded form is 'foo%3Dbar' and in base64 encoding is 'Zm9vJTI1M0RiYXI='.</rdfs:comment>
    <rdfs:domain rdf:resource="http://example.org/onto/class/google_monitoring_uptime_check_config"/>
    <rdfs:range rdf:resource="http://www.w3.org/2001/XMLSchema#string"/>
  </owl:DatatypeProperty>
  <owl:DatatypeProperty rdf:about="http://example.org/onto/prop/google_monitoring_uptime_check_config_content_type">
    <rdfs:label>content_type</rdfs:label>
    <rdfs:comment>The content type to use for the check. Possible values: ["TYPE_UNSPECIFIED", "URL_ENCODED", "USER_PROVIDED"]</rdfs:comment>
    <rdfs:domain rdf:resource="http://example.org/onto/class/google_monitoring_uptime_check_config"/>
    <rdfs:range rdf:resource="http://www.w3.org/2001/XMLSchema#string"/>
  </owl:DatatypeProperty>
  <owl:DatatypeProperty rdf:about="http://example.org/onto/prop/google_monitoring_uptime_check_config_custom_content_type">
    <rdfs:label>custom_content_type</rdfs:label>
    <rdfs:comment>A user provided content type header to use for the check. The invalid configurations outlined in the 'content_type' field apply to custom_content_type', as well as the following 1. 'content_type' is 'URL_ENCODED' and 'custom_content_type' is set. 2. 'content_type' is 'USER_PROVIDED' and 'custom_content_type' is not set.</rdfs:comment>
    <rdfs:domain rdf:resource="http://example.org/onto/class/google_monitoring_uptime_check_config"/>
    <rdfs:range rdf:resource="http://www.w3.org/2001/XMLSchema#string"/>
  </owl:DatatypeProperty>
  <owl:DatatypeProperty rdf:about="http://example.org/onto/prop/google_monitoring_uptime_check_config_headers">
    <rdfs:label>headers</rdfs:label>
    <rdfs:comment>The list of headers to send as part of the uptime check request. If two headers have the same key and different values, they should be entered as a single header, with the value being a comma-separated list of all the desired values as described in [RFC 2616 (page 31)](https://www.w3.org/Protocols/rfc2616/rfc2616.txt). Entering two separate headers with the same key in a Create call will cause the first to be overwritten by the second. The maximum number of headers allowed is 100.</rdfs:comment>
    <rdfs:domain rdf:resource="http://example.org/onto/class/google_monitoring_uptime_check_config"/>
    <rdfs:range rdf:resource="http://www.w3.org/2001/XMLSchema#string"/>
  </owl:DatatypeProperty>
  <owl:DatatypeProperty rdf:about="http://example.org/onto/prop/google_monitoring_uptime_check_config_mask_headers">
    <rdfs:label>mask_headers</rdfs:label>
    <rdfs:comment>Boolean specifying whether to encrypt the header information. Encryption should be specified for any headers related to authentication that you do not wish to be seen when retrieving the configuration. The server will be responsible for encrypting the headers. On Get/List calls, if 'mask_headers' is set to 'true' then the headers will be obscured with '******'.</rdfs:comment>
    <rdfs:domain rdf:resource="http://example.org/onto/class/google_monitoring_uptime_check_config"/>
    <rdfs:range rdf:resource="http://www.w3.org/2001/XMLSchema#string"/>
  </owl:DatatypeProperty>
  <owl:DatatypeProperty rdf:about="http://example.org/onto/prop/google_monitoring_uptime_check_config_path">
    <rdfs:label>path</rdfs:label>
    <rdfs:comment>The path to the page to run the check against. Will be combined with the host (specified within the MonitoredResource) and port to construct the full URL. If the provided path does not begin with '/', a '/' will be prepended automatically. Optional (defaults to '/').</rdfs:comment>
    <rdfs:domain rdf:resource="http://example.org/onto/class/google_monitoring_uptime_check_config"/>
    <rdfs:range rdf:resource="http://www.w3.org/2001/XMLSchema#string"/>
  </owl:DatatypeProperty>
  <owl:DatatypeProperty rdf:about="http://example.org/onto/prop/google_monitoring_uptime_check_config_port">
    <rdfs:label>port</rdfs:label>
    <rdfs:comment>The port to the page to run the check against. Will be combined with 'host' (specified within the ['monitored_resource'](#nested_monitored_resource)) and path to construct the full URL. Optional (defaults to 80 without SSL, or 443 with SSL).</rdfs:comment>
    <rdfs:domain rdf:resource="http://example.org/onto/class/google_monitoring_uptime_check_config"/>
    <rdfs:range rdf:resource="http://www.w3.org/2001/XMLSchema#string"/>
  </owl:DatatypeProperty>
  <owl:DatatypeProperty rdf:about="http://example.org/onto/prop/google_monitoring_uptime_check_config_request_method">
    <rdfs:label>request_method</rdfs:label>
    <rdfs:comment>The HTTP request method to use for the check. If set to 'METHOD_UNSPECIFIED' then 'request_method' defaults to 'GET'. Default value: "GET" Possible values: ["METHOD_UNSPECIFIED", "GET", "POST"]</rdfs:comment>
    <rdfs:domain rdf:resource="http://example.org/onto/class/google_monitoring_uptime_check_config"/>
    <rdfs:range rdf:resource="http://www.w3.org/2001/XMLSchema#string"/>
  </owl:DatatypeProperty>
  <owl:DatatypeProperty rdf:about="http://example.org/onto/prop/google_monitoring_uptime_check_config_use_ssl">
    <rdfs:label>use_ssl</rdfs:label>
    <rdfs:comment>If true, use HTTPS instead of HTTP to run the check.</rdfs:comment>
    <rdfs:domain rdf:resource="http://example.org/onto/class/google_monitoring_uptime_check_config"/>
    <rdfs:range rdf:resource="http://www.w3.org/2001/XMLSchema#string"/>
  </owl:DatatypeProperty>
  <owl:DatatypeProperty rdf:about="http://example.org/onto/prop/google_monitoring_uptime_check_config_validate_ssl">
    <rdfs:label>validate_ssl</rdfs:label>
    <rdfs:comment>Boolean specifying whether to include SSL certificate validation as a part of the Uptime check. Only applies to checks where 'monitored_resource' is set to 'uptime_url'. If 'use_ssl' is 'false', setting 'validate_ssl' to 'true' has no effect.</rdfs:comment>
    <rdfs:domain rdf:resource="http://example.org/onto/class/google_monitoring_uptime_check_config"/>
    <rdfs:range rdf:resource="http://www.w3.org/2001/XMLSchema#string"/>
  </owl:DatatypeProperty>
  <owl:DatatypeProperty rdf:about="http://example.org/onto/prop/google_monitoring_uptime_check_config_status_class">
    <rdfs:label>status_class</rdfs:label>
    <rdfs:comment>A class of status codes to accept. Possible values: ["STATUS_CLASS_1XX", "STATUS_CLASS_2XX", "STATUS_CLASS_3XX", "STATUS_CLASS_4XX", "STATUS_CLASS_5XX", "STATUS_CLASS_ANY"]</rdfs:comment>
    <rdfs:domain rdf:resource="http://example.org/onto/class/google_monitoring_uptime_check_config"/>
    <rdfs:range rdf:resource="http://www.w3.org/2001/XMLSchema#string"/>
  </owl:DatatypeProperty>
  <owl:DatatypeProperty rdf:about="http://example.org/onto/prop/google_monitoring_uptime_check_config_status_value">
    <rdfs:label>status_value</rdfs:label>
    <rdfs:comment>A status code to accept.</rdfs:comment>
    <rdfs:domain rdf:resource="http://example.org/onto/class/google_monitoring_uptime_check_config"/>
    <rdfs:range rdf:resource="http://www.w3.org/2001/XMLSchema#string"/>
  </owl:DatatypeProperty>
  <owl:DatatypeProperty rdf:about="http://example.org/onto/prop/google_monitoring_uptime_check_config_password">
    <rdfs:label>password</rdfs:label>
    <rdfs:comment>The password to authenticate.</rdfs:comment>
    <rdfs:domain rdf:resource="http://example.org/onto/class/google_monitoring_uptime_check_config"/>
    <rdfs:range rdf:resource="http://www.w3.org/2001/XMLSchema#string"/>
  </owl:DatatypeProperty>
  <owl:DatatypeProperty rdf:about="http://example.org/onto/prop/google_monitoring_uptime_check_config_password_wo">
    <rdfs:label>password_wo</rdfs:label>
    <rdfs:comment>The password to authenticate.</rdfs:comment>
    <rdfs:domain rdf:resource="http://example.org/onto/class/google_monitoring_uptime_check_config"/>
    <rdfs:range rdf:resource="http://www.w3.org/2001/XMLSchema#string"/>
  </owl:DatatypeProperty>
  <owl:DatatypeProperty rdf:about="http://example.org/onto/prop/google_monitoring_uptime_check_config_password_wo_version">
    <rdfs:label>password_wo_version</rdfs:label>
    <rdfs:comment>The password write-only version.</rdfs:comment>
    <rdfs:domain rdf:resource="http://example.org/onto/class/google_monitoring_uptime_check_config"/>
    <rdfs:range rdf:resource="http://www.w3.org/2001/XMLSchema#string"/>
  </owl:DatatypeProperty>
  <owl:DatatypeProperty rdf:about="http://example.org/onto/prop/google_monitoring_uptime_check_config_username">
    <rdfs:label>username</rdfs:label>
    <rdfs:comment>The username to authenticate.</rdfs:comment>
    <rdfs:domain rdf:resource="http://example.org/onto/class/google_monitoring_uptime_check_config"/>
    <rdfs:range rdf:resource="http://www.w3.org/2001/XMLSchema#string"/>
  </owl:DatatypeProperty>
  <owl:DatatypeProperty rdf:about="http://example.org/onto/prop/google_monitoring_uptime_check_config_pings_count">
    <rdfs:label>pings_count</rdfs:label>
    <rdfs:comment>Number of ICMP pings. A maximum of 3 ICMP pings is currently supported.</rdfs:comment>
    <rdfs:domain rdf:resource="http://example.org/onto/class/google_monitoring_uptime_check_config"/>
    <rdfs:range rdf:resource="http://www.w3.org/2001/XMLSchema#string"/>
  </owl:DatatypeProperty>
  <owl:DatatypeProperty rdf:about="http://example.org/onto/prop/google_monitoring_uptime_check_config_type">
    <rdfs:label>type</rdfs:label>
    <rdfs:comment>The type of authentication to use. Possible values: ["SERVICE_AGENT_AUTHENTICATION_TYPE_UNSPECIFIED", "OIDC_TOKEN"]</rdfs:comment>
    <rdfs:domain rdf:resource="http://example.org/onto/class/google_monitoring_uptime_check_config"/>
    <rdfs:range rdf:resource="http://www.w3.org/2001/XMLSchema#string"/>
  </owl:DatatypeProperty>
  <owl:DatatypeProperty rdf:about="http://example.org/onto/prop/google_monitoring_uptime_check_config_labels">
    <rdfs:label>labels</rdfs:label>
    <rdfs:comment>Values for all of the labels listed in the associated monitored resource descriptor. For example, Compute Engine VM instances use the labels 'project_id', 'instance_id', and 'zone'.</rdfs:comment>
    <rdfs:domain rdf:resource="http://example.org/onto/class/google_monitoring_uptime_check_config"/>
    <rdfs:range rdf:resource="http://www.w3.org/2001/XMLSchema#string"/>
  </owl:DatatypeProperty>
  <owl:DatatypeProperty rdf:about="http://example.org/onto/prop/google_monitoring_uptime_check_config_type">
    <rdfs:label>type</rdfs:label>
    <rdfs:comment>The monitored resource type. This field must match the type field of a ['MonitoredResourceDescriptor'](https://cloud.google.com/monitoring/api/ref_v3/rest/v3/projects.monitoredResourceDescriptors#MonitoredResourceDescriptor) object. For example, the type of a Compute Engine VM instance is 'gce_instance'. For a list of types, see [Monitoring resource types](https://cloud.google.com/monitoring/api/resources) and [Logging resource types](https://cloud.google.com/logging/docs/api/v2/resource-list).</rdfs:comment>
    <rdfs:domain rdf:resource="http://example.org/onto/class/google_monitoring_uptime_check_config"/>
    <rdfs:range rdf:resource="http://www.w3.org/2001/XMLSchema#string"/>
  </owl:DatatypeProperty>
  <owl:DatatypeProperty rdf:about="http://example.org/onto/prop/google_monitoring_uptime_check_config_group_id">
    <rdfs:label>group_id</rdfs:label>
    <rdfs:comment>The group of resources being monitored. Should be the 'name' of a group</rdfs:comment>
    <rdfs:domain rdf:resource="http://example.org/onto/class/google_monitoring_uptime_check_config"/>
    <rdfs:range rdf:resource="http://www.w3.org/2001/XMLSchema#string"/>
  </owl:DatatypeProperty>
  <owl:DatatypeProperty rdf:about="http://example.org/onto/prop/google_monitoring_uptime_check_config_resource_type">
    <rdfs:label>resource_type</rdfs:label>
    <rdfs:comment>The resource type of the group members. Possible values: ["RESOURCE_TYPE_UNSPECIFIED", "INSTANCE", "AWS_ELB_LOAD_BALANCER"]</rdfs:comment>
    <rdfs:domain rdf:resource="http://example.org/onto/class/google_monitoring_uptime_check_config"/>
    <rdfs:range rdf:resource="http://www.w3.org/2001/XMLSchema#string"/>
  </owl:DatatypeProperty>
  <owl:DatatypeProperty rdf:about="http://example.org/onto/prop/google_monitoring_uptime_check_config_name">
    <rdfs:label>name</rdfs:label>
    <rdfs:comment>The fully qualified name of the cloud function resource.</rdfs:comment>
    <rdfs:domain rdf:resource="http://example.org/onto/class/google_monitoring_uptime_check_config"/>
    <rdfs:range rdf:resource="http://www.w3.org/2001/XMLSchema#string"/>
  </owl:DatatypeProperty>
  <owl:DatatypeProperty rdf:about="http://example.org/onto/prop/google_monitoring_uptime_check_config_port">
    <rdfs:label>port</rdfs:label>
    <rdfs:comment>The port to the page to run the check against. Will be combined with host (specified within the 'monitored_resource') to construct the full URL.</rdfs:comment>
    <rdfs:domain rdf:resource="http://example.org/onto/class/google_monitoring_uptime_check_config"/>
    <rdfs:range rdf:resource="http://www.w3.org/2001/XMLSchema#string"/>
  </owl:DatatypeProperty>
  <owl:DatatypeProperty rdf:about="http://example.org/onto/prop/google_monitoring_uptime_check_config_pings_count">
    <rdfs:label>pings_count</rdfs:label>
    <rdfs:comment>Number of ICMP pings. A maximum of 3 ICMP pings is currently supported.</rdfs:comment>
    <rdfs:domain rdf:resource="http://example.org/onto/class/google_monitoring_uptime_check_config"/>
    <rdfs:range rdf:resource="http://www.w3.org/2001/XMLSchema#string"/>
  </owl:DatatypeProperty>
  <owl:DatatypeProperty rdf:about="http://example.org/onto/prop/google_monitoring_uptime_check_config_create">
    <rdfs:label>create</rdfs:label>
    <rdfs:domain rdf:resource="http://example.org/onto/class/google_monitoring_uptime_check_config"/>
    <rdfs:range rdf:resource="http://www.w3.org/2001/XMLSchema#string"/>
  </owl:DatatypeProperty>
  <owl:DatatypeProperty rdf:about="http://example.org/onto/prop/google_monitoring_uptime_check_config_delete">
    <rdfs:label>delete</rdfs:label>
    <rdfs:domain rdf:resource="http://example.org/onto/class/google_monitoring_uptime_check_config"/>
    <rdfs:range rdf:resource="http://www.w3.org/2001/XMLSchema#string"/>
  </owl:DatatypeProperty>
  <owl:DatatypeProperty rdf:about="http://example.org/onto/prop/google_monitoring_uptime_check_config_update">
    <rdfs:label>update</rdfs:label>
    <rdfs:domain rdf:resource="http://example.org/onto/class/google_monitoring_uptime_check_config"/>
    <rdfs:range rdf:resource="http://www.w3.org/2001/XMLSchema#string"/>
  </owl:DatatypeProperty>
</rdf:RDF>
