<?xml version="1.0" encoding="UTF-8"?>
<rdf:RDF
  xmlns:rdf="http://www.w3.org/1999/02/22-rdf-syntax-ns#"
  xmlns:rdfs="http://www.w3.org/2000/01/rdf-schema#"
  xmlns:owl="http://www.w3.org/2002/07/owl#"
  xmlns:xsd="http://www.w3.org/2001/XMLSchema#"
  xml:base="http://example.org/onto/">
  <owl:Class rdf:about="http://example.org/onto/class/google_compute_region_network_firewall_policy_with_rules">
    <rdfs:label>google_compute_region_network_firewall_policy_with_rules</rdfs:label>
    <rdfs:comment>#
#     ***     AUTO GENERATED CODE    ***    Type: MMv1     ***
#
# ----------------------------------------------------------------------------
#
#     This code is generated by Magic Modules using the following:
#
#     Configuration: https:#github.com/GoogleCloudPlatform/magic-modules/tree/main/mmv1/products/compute/RegionNetworkFirewallPolicyWithRules.yaml
#     Template:      https:#github.com/GoogleCloudPlatform/magic-modules/tree/main/mmv1/templates/terraform/resource.html.markdown.tmpl
#
#     DO NOT EDIT this file directly. Any changes made to this file will be
#     overwritten during the next generation cycle.
#
# ----------------------------------------------------------------------------
subcategory: "Compute Engine"
description: |-
  The Compute NetworkFirewallPolicy with rules resource
---</rdfs:comment>
  </owl:Class>
  <owl:DatatypeProperty rdf:about="http://example.org/onto/prop/google_compute_region_network_firewall_policy_with_rules_creation_timestamp">
    <rdfs:label>creation_timestamp</rdfs:label>
    <rdfs:comment>Creation timestamp in RFC3339 text format.</rdfs:comment>
    <rdfs:domain rdf:resource="http://example.org/onto/class/google_compute_region_network_firewall_policy_with_rules"/>
    <rdfs:range rdf:resource="http://www.w3.org/2001/XMLSchema#string"/>
  </owl:DatatypeProperty>
  <owl:DatatypeProperty rdf:about="http://example.org/onto/prop/google_compute_region_network_firewall_policy_with_rules_description">
    <rdfs:label>description</rdfs:label>
    <rdfs:comment>An optional description of this resource.</rdfs:comment>
    <rdfs:domain rdf:resource="http://example.org/onto/class/google_compute_region_network_firewall_policy_with_rules"/>
    <rdfs:range rdf:resource="http://www.w3.org/2001/XMLSchema#string"/>
  </owl:DatatypeProperty>
  <owl:DatatypeProperty rdf:about="http://example.org/onto/prop/google_compute_region_network_firewall_policy_with_rules_fingerprint">
    <rdfs:label>fingerprint</rdfs:label>
    <rdfs:comment>Fingerprint of the resource. This field is used internally during updates of this resource.</rdfs:comment>
    <rdfs:domain rdf:resource="http://example.org/onto/class/google_compute_region_network_firewall_policy_with_rules"/>
    <rdfs:range rdf:resource="http://www.w3.org/2001/XMLSchema#string"/>
  </owl:DatatypeProperty>
  <owl:DatatypeProperty rdf:about="http://example.org/onto/prop/google_compute_region_network_firewall_policy_with_rules_id">
    <rdfs:label>id</rdfs:label>
    <rdfs:domain rdf:resource="http://example.org/onto/class/google_compute_region_network_firewall_policy_with_rules"/>
    <rdfs:range rdf:resource="http://www.w3.org/2001/XMLSchema#string"/>
  </owl:DatatypeProperty>
  <owl:DatatypeProperty rdf:about="http://example.org/onto/prop/google_compute_region_network_firewall_policy_with_rules_name">
    <rdfs:label>name</rdfs:label>
    <rdfs:comment>User-provided name of the Network firewall policy.
The name should be unique in the project in which the firewall policy is created.
The name must be 1-63 characters long, and comply with RFC1035. Specifically,
the name must be 1-63 characters long and match the regular expression [a-z]([-a-z0-9]*[a-z0-9])?
which means the first character must be a lowercase letter, and all following characters must be a dash,
lowercase letter, or digit, except the last character, which cannot be a dash.</rdfs:comment>
    <rdfs:domain rdf:resource="http://example.org/onto/class/google_compute_region_network_firewall_policy_with_rules"/>
    <rdfs:range rdf:resource="http://www.w3.org/2001/XMLSchema#string"/>
  </owl:DatatypeProperty>
  <owl:DatatypeProperty rdf:about="http://example.org/onto/prop/google_compute_region_network_firewall_policy_with_rules_network_firewall_policy_id">
    <rdfs:label>network_firewall_policy_id</rdfs:label>
    <rdfs:comment>The unique identifier for the resource. This identifier is defined by the server.</rdfs:comment>
    <rdfs:domain rdf:resource="http://example.org/onto/class/google_compute_region_network_firewall_policy_with_rules"/>
    <rdfs:range rdf:resource="http://www.w3.org/2001/XMLSchema#string"/>
  </owl:DatatypeProperty>
  <owl:DatatypeProperty rdf:about="http://example.org/onto/prop/google_compute_region_network_firewall_policy_with_rules_predefined_rules">
    <rdfs:label>predefined_rules</rdfs:label>
    <rdfs:comment>A list of firewall policy pre-defined rules.</rdfs:comment>
    <rdfs:domain rdf:resource="http://example.org/onto/class/google_compute_region_network_firewall_policy_with_rules"/>
    <rdfs:range rdf:resource="http://www.w3.org/2001/XMLSchema#string"/>
  </owl:DatatypeProperty>
  <owl:DatatypeProperty rdf:about="http://example.org/onto/prop/google_compute_region_network_firewall_policy_with_rules_project">
    <rdfs:label>project</rdfs:label>
    <rdfs:domain rdf:resource="http://example.org/onto/class/google_compute_region_network_firewall_policy_with_rules"/>
    <rdfs:range rdf:resource="http://www.w3.org/2001/XMLSchema#string"/>
  </owl:DatatypeProperty>
  <owl:DatatypeProperty rdf:about="http://example.org/onto/prop/google_compute_region_network_firewall_policy_with_rules_region">
    <rdfs:label>region</rdfs:label>
    <rdfs:comment>The region of this resource.</rdfs:comment>
    <rdfs:domain rdf:resource="http://example.org/onto/class/google_compute_region_network_firewall_policy_with_rules"/>
    <rdfs:range rdf:resource="http://www.w3.org/2001/XMLSchema#string"/>
  </owl:DatatypeProperty>
  <owl:DatatypeProperty rdf:about="http://example.org/onto/prop/google_compute_region_network_firewall_policy_with_rules_rule_tuple_count">
    <rdfs:label>rule_tuple_count</rdfs:label>
    <rdfs:comment>Total count of all firewall policy rule tuples. A firewall policy can not exceed a set number of tuples.</rdfs:comment>
    <rdfs:domain rdf:resource="http://example.org/onto/class/google_compute_region_network_firewall_policy_with_rules"/>
    <rdfs:range rdf:resource="http://www.w3.org/2001/XMLSchema#string"/>
  </owl:DatatypeProperty>
  <owl:DatatypeProperty rdf:about="http://example.org/onto/prop/google_compute_region_network_firewall_policy_with_rules_self_link">
    <rdfs:label>self_link</rdfs:label>
    <rdfs:comment>Server-defined URL for the resource.</rdfs:comment>
    <rdfs:domain rdf:resource="http://example.org/onto/class/google_compute_region_network_firewall_policy_with_rules"/>
    <rdfs:range rdf:resource="http://www.w3.org/2001/XMLSchema#string"/>
  </owl:DatatypeProperty>
  <owl:DatatypeProperty rdf:about="http://example.org/onto/prop/google_compute_region_network_firewall_policy_with_rules_self_link_with_id">
    <rdfs:label>self_link_with_id</rdfs:label>
    <rdfs:comment>Server-defined URL for this resource with the resource id.</rdfs:comment>
    <rdfs:domain rdf:resource="http://example.org/onto/class/google_compute_region_network_firewall_policy_with_rules"/>
    <rdfs:range rdf:resource="http://www.w3.org/2001/XMLSchema#string"/>
  </owl:DatatypeProperty>
  <owl:DatatypeProperty rdf:about="http://example.org/onto/prop/google_compute_region_network_firewall_policy_with_rules_action">
    <rdfs:label>action</rdfs:label>
    <rdfs:comment>The Action to perform when the client connection triggers the rule. Can currently be either
"allow", "deny", "apply_security_profile_group" or "goto_next".</rdfs:comment>
    <rdfs:domain rdf:resource="http://example.org/onto/class/google_compute_region_network_firewall_policy_with_rules"/>
    <rdfs:range rdf:resource="http://www.w3.org/2001/XMLSchema#string"/>
  </owl:DatatypeProperty>
  <owl:DatatypeProperty rdf:about="http://example.org/onto/prop/google_compute_region_network_firewall_policy_with_rules_description">
    <rdfs:label>description</rdfs:label>
    <rdfs:comment>A description of the rule.</rdfs:comment>
    <rdfs:domain rdf:resource="http://example.org/onto/class/google_compute_region_network_firewall_policy_with_rules"/>
    <rdfs:range rdf:resource="http://www.w3.org/2001/XMLSchema#string"/>
  </owl:DatatypeProperty>
  <owl:DatatypeProperty rdf:about="http://example.org/onto/prop/google_compute_region_network_firewall_policy_with_rules_direction">
    <rdfs:label>direction</rdfs:label>
    <rdfs:comment>The direction in which this rule applies. If unspecified an INGRESS rule is created. Possible values: ["INGRESS", "EGRESS"]</rdfs:comment>
    <rdfs:domain rdf:resource="http://example.org/onto/class/google_compute_region_network_firewall_policy_with_rules"/>
    <rdfs:range rdf:resource="http://www.w3.org/2001/XMLSchema#string"/>
  </owl:DatatypeProperty>
  <owl:DatatypeProperty rdf:about="http://example.org/onto/prop/google_compute_region_network_firewall_policy_with_rules_disabled">
    <rdfs:label>disabled</rdfs:label>
    <rdfs:comment>Denotes whether the firewall policy rule is disabled. When set to true,
the firewall policy rule is not enforced and traffic behaves as if it did
not exist. If this is unspecified, the firewall policy rule will be
enabled.</rdfs:comment>
    <rdfs:domain rdf:resource="http://example.org/onto/class/google_compute_region_network_firewall_policy_with_rules"/>
    <rdfs:range rdf:resource="http://www.w3.org/2001/XMLSchema#string"/>
  </owl:DatatypeProperty>
  <owl:DatatypeProperty rdf:about="http://example.org/onto/prop/google_compute_region_network_firewall_policy_with_rules_enable_logging">
    <rdfs:label>enable_logging</rdfs:label>
    <rdfs:comment>Denotes whether to enable logging for a particular rule.
If logging is enabled, logs will be exported to the
configured export destination in Stackdriver.</rdfs:comment>
    <rdfs:domain rdf:resource="http://example.org/onto/class/google_compute_region_network_firewall_policy_with_rules"/>
    <rdfs:range rdf:resource="http://www.w3.org/2001/XMLSchema#string"/>
  </owl:DatatypeProperty>
  <owl:DatatypeProperty rdf:about="http://example.org/onto/prop/google_compute_region_network_firewall_policy_with_rules_priority">
    <rdfs:label>priority</rdfs:label>
    <rdfs:comment>An integer indicating the priority of a rule in the list. The priority must be a value
between 0 and 2147483647. Rules are evaluated from highest to lowest priority where 0 is the
highest priority and 2147483647 is the lowest priority.</rdfs:comment>
    <rdfs:domain rdf:resource="http://example.org/onto/class/google_compute_region_network_firewall_policy_with_rules"/>
    <rdfs:range rdf:resource="http://www.w3.org/2001/XMLSchema#string"/>
  </owl:DatatypeProperty>
  <owl:DatatypeProperty rdf:about="http://example.org/onto/prop/google_compute_region_network_firewall_policy_with_rules_rule_name">
    <rdfs:label>rule_name</rdfs:label>
    <rdfs:comment>An optional name for the rule. This field is not a unique identifier
and can be updated.</rdfs:comment>
    <rdfs:domain rdf:resource="http://example.org/onto/class/google_compute_region_network_firewall_policy_with_rules"/>
    <rdfs:range rdf:resource="http://www.w3.org/2001/XMLSchema#string"/>
  </owl:DatatypeProperty>
  <owl:DatatypeProperty rdf:about="http://example.org/onto/prop/google_compute_region_network_firewall_policy_with_rules_security_profile_group">
    <rdfs:label>security_profile_group</rdfs:label>
    <rdfs:comment>A fully-qualified URL of a SecurityProfile resource instance.
Example:
https://networksecurity.googleapis.com/v1/projects/{project}/locations/{location}/securityProfileGroups/my-security-profile-group
Must be specified if action is 'apply_security_profile_group'.</rdfs:comment>
    <rdfs:domain rdf:resource="http://example.org/onto/class/google_compute_region_network_firewall_policy_with_rules"/>
    <rdfs:range rdf:resource="http://www.w3.org/2001/XMLSchema#string"/>
  </owl:DatatypeProperty>
  <owl:DatatypeProperty rdf:about="http://example.org/onto/prop/google_compute_region_network_firewall_policy_with_rules_target_service_accounts">
    <rdfs:label>target_service_accounts</rdfs:label>
    <rdfs:comment>A list of service accounts indicating the sets of
instances that are applied with this rule.</rdfs:comment>
    <rdfs:domain rdf:resource="http://example.org/onto/class/google_compute_region_network_firewall_policy_with_rules"/>
    <rdfs:range rdf:resource="http://www.w3.org/2001/XMLSchema#string"/>
  </owl:DatatypeProperty>
  <owl:DatatypeProperty rdf:about="http://example.org/onto/prop/google_compute_region_network_firewall_policy_with_rules_tls_inspect">
    <rdfs:label>tls_inspect</rdfs:label>
    <rdfs:comment>Boolean flag indicating if the traffic should be TLS decrypted.
It can be set only if action = 'apply_security_profile_group' and cannot be set for other actions.</rdfs:comment>
    <rdfs:domain rdf:resource="http://example.org/onto/class/google_compute_region_network_firewall_policy_with_rules"/>
    <rdfs:range rdf:resource="http://www.w3.org/2001/XMLSchema#string"/>
  </owl:DatatypeProperty>
  <owl:DatatypeProperty rdf:about="http://example.org/onto/prop/google_compute_region_network_firewall_policy_with_rules_dest_address_groups">
    <rdfs:label>dest_address_groups</rdfs:label>
    <rdfs:comment>Address groups which should be matched against the traffic destination.
Maximum number of destination address groups is 10.</rdfs:comment>
    <rdfs:domain rdf:resource="http://example.org/onto/class/google_compute_region_network_firewall_policy_with_rules"/>
    <rdfs:range rdf:resource="http://www.w3.org/2001/XMLSchema#string"/>
  </owl:DatatypeProperty>
  <owl:DatatypeProperty rdf:about="http://example.org/onto/prop/google_compute_region_network_firewall_policy_with_rules_dest_fqdns">
    <rdfs:label>dest_fqdns</rdfs:label>
    <rdfs:comment>Fully Qualified Domain Name (FQDN) which should be matched against
traffic destination. Maximum number of destination fqdn allowed is 100.</rdfs:comment>
    <rdfs:domain rdf:resource="http://example.org/onto/class/google_compute_region_network_firewall_policy_with_rules"/>
    <rdfs:range rdf:resource="http://www.w3.org/2001/XMLSchema#string"/>
  </owl:DatatypeProperty>
  <owl:DatatypeProperty rdf:about="http://example.org/onto/prop/google_compute_region_network_firewall_policy_with_rules_dest_ip_ranges">
    <rdfs:label>dest_ip_ranges</rdfs:label>
    <rdfs:comment>Destination IP address range in CIDR format. Required for
EGRESS rules.</rdfs:comment>
    <rdfs:domain rdf:resource="http://example.org/onto/class/google_compute_region_network_firewall_policy_with_rules"/>
    <rdfs:range rdf:resource="http://www.w3.org/2001/XMLSchema#string"/>
  </owl:DatatypeProperty>
  <owl:DatatypeProperty rdf:about="http://example.org/onto/prop/google_compute_region_network_firewall_policy_with_rules_dest_region_codes">
    <rdfs:label>dest_region_codes</rdfs:label>
    <rdfs:comment>Region codes whose IP addresses will be used to match for destination
of traffic. Should be specified as 2 letter country code defined as per
ISO 3166 alpha-2 country codes. ex."US"
Maximum number of destination region codes allowed is 5000.</rdfs:comment>
    <rdfs:domain rdf:resource="http://example.org/onto/class/google_compute_region_network_firewall_policy_with_rules"/>
    <rdfs:range rdf:resource="http://www.w3.org/2001/XMLSchema#string"/>
  </owl:DatatypeProperty>
  <owl:DatatypeProperty rdf:about="http://example.org/onto/prop/google_compute_region_network_firewall_policy_with_rules_dest_threat_intelligences">
    <rdfs:label>dest_threat_intelligences</rdfs:label>
    <rdfs:comment>Names of Network Threat Intelligence lists.
The IPs in these lists will be matched against traffic destination.</rdfs:comment>
    <rdfs:domain rdf:resource="http://example.org/onto/class/google_compute_region_network_firewall_policy_with_rules"/>
    <rdfs:range rdf:resource="http://www.w3.org/2001/XMLSchema#string"/>
  </owl:DatatypeProperty>
  <owl:DatatypeProperty rdf:about="http://example.org/onto/prop/google_compute_region_network_firewall_policy_with_rules_src_address_groups">
    <rdfs:label>src_address_groups</rdfs:label>
    <rdfs:comment>Address groups which should be matched against the traffic source.
Maximum number of source address groups is 10.</rdfs:comment>
    <rdfs:domain rdf:resource="http://example.org/onto/class/google_compute_region_network_firewall_policy_with_rules"/>
    <rdfs:range rdf:resource="http://www.w3.org/2001/XMLSchema#string"/>
  </owl:DatatypeProperty>
  <owl:DatatypeProperty rdf:about="http://example.org/onto/prop/google_compute_region_network_firewall_policy_with_rules_src_fqdns">
    <rdfs:label>src_fqdns</rdfs:label>
    <rdfs:comment>Fully Qualified Domain Name (FQDN) which should be matched against
traffic source. Maximum number of source fqdn allowed is 100.</rdfs:comment>
    <rdfs:domain rdf:resource="http://example.org/onto/class/google_compute_region_network_firewall_policy_with_rules"/>
    <rdfs:range rdf:resource="http://www.w3.org/2001/XMLSchema#string"/>
  </owl:DatatypeProperty>
  <owl:DatatypeProperty rdf:about="http://example.org/onto/prop/google_compute_region_network_firewall_policy_with_rules_src_ip_ranges">
    <rdfs:label>src_ip_ranges</rdfs:label>
    <rdfs:comment>Source IP address range in CIDR format. Required for
INGRESS rules.</rdfs:comment>
    <rdfs:domain rdf:resource="http://example.org/onto/class/google_compute_region_network_firewall_policy_with_rules"/>
    <rdfs:range rdf:resource="http://www.w3.org/2001/XMLSchema#string"/>
  </owl:DatatypeProperty>
  <owl:DatatypeProperty rdf:about="http://example.org/onto/prop/google_compute_region_network_firewall_policy_with_rules_src_region_codes">
    <rdfs:label>src_region_codes</rdfs:label>
    <rdfs:comment>Region codes whose IP addresses will be used to match for source
of traffic. Should be specified as 2 letter country code defined as per
ISO 3166 alpha-2 country codes. ex."US"
Maximum number of source region codes allowed is 5000.</rdfs:comment>
    <rdfs:domain rdf:resource="http://example.org/onto/class/google_compute_region_network_firewall_policy_with_rules"/>
    <rdfs:range rdf:resource="http://www.w3.org/2001/XMLSchema#string"/>
  </owl:DatatypeProperty>
  <owl:DatatypeProperty rdf:about="http://example.org/onto/prop/google_compute_region_network_firewall_policy_with_rules_src_threat_intelligences">
    <rdfs:label>src_threat_intelligences</rdfs:label>
    <rdfs:comment>Names of Network Threat Intelligence lists.
The IPs in these lists will be matched against traffic source.</rdfs:comment>
    <rdfs:domain rdf:resource="http://example.org/onto/class/google_compute_region_network_firewall_policy_with_rules"/>
    <rdfs:range rdf:resource="http://www.w3.org/2001/XMLSchema#string"/>
  </owl:DatatypeProperty>
  <owl:DatatypeProperty rdf:about="http://example.org/onto/prop/google_compute_region_network_firewall_policy_with_rules_ip_protocol">
    <rdfs:label>ip_protocol</rdfs:label>
    <rdfs:comment>The IP protocol to which this rule applies. The protocol
type is required when creating a firewall rule.
This value can either be one of the following well
known protocol strings (tcp, udp, icmp, esp, ah, ipip, sctp),
or the IP protocol number.</rdfs:comment>
    <rdfs:domain rdf:resource="http://example.org/onto/class/google_compute_region_network_firewall_policy_with_rules"/>
    <rdfs:range rdf:resource="http://www.w3.org/2001/XMLSchema#string"/>
  </owl:DatatypeProperty>
  <owl:DatatypeProperty rdf:about="http://example.org/onto/prop/google_compute_region_network_firewall_policy_with_rules_ports">
    <rdfs:label>ports</rdfs:label>
    <rdfs:comment>An optional list of ports to which this rule applies. This field
is only applicable for UDP or TCP protocol. Each entry must be
either an integer or a range. If not specified, this rule
applies to connections through any port.
Example inputs include: ["22"], ["80","443"], and
["12345-12349"].</rdfs:comment>
    <rdfs:domain rdf:resource="http://example.org/onto/class/google_compute_region_network_firewall_policy_with_rules"/>
    <rdfs:range rdf:resource="http://www.w3.org/2001/XMLSchema#string"/>
  </owl:DatatypeProperty>
  <owl:DatatypeProperty rdf:about="http://example.org/onto/prop/google_compute_region_network_firewall_policy_with_rules_name">
    <rdfs:label>name</rdfs:label>
    <rdfs:comment>Name of the secure tag, created with TagManager's TagValue API.
@pattern tagValues/[0-9]+</rdfs:comment>
    <rdfs:domain rdf:resource="http://example.org/onto/class/google_compute_region_network_firewall_policy_with_rules"/>
    <rdfs:range rdf:resource="http://www.w3.org/2001/XMLSchema#string"/>
  </owl:DatatypeProperty>
  <owl:DatatypeProperty rdf:about="http://example.org/onto/prop/google_compute_region_network_firewall_policy_with_rules_state">
    <rdfs:label>state</rdfs:label>
    <rdfs:comment>[Output Only] State of the secure tag, either 'EFFECTIVE' or
'INEFFECTIVE'. A secure tag is 'INEFFECTIVE' when it is deleted
or its network is deleted.</rdfs:comment>
    <rdfs:domain rdf:resource="http://example.org/onto/class/google_compute_region_network_firewall_policy_with_rules"/>
    <rdfs:range rdf:resource="http://www.w3.org/2001/XMLSchema#string"/>
  </owl:DatatypeProperty>
  <owl:DatatypeProperty rdf:about="http://example.org/onto/prop/google_compute_region_network_firewall_policy_with_rules_name">
    <rdfs:label>name</rdfs:label>
    <rdfs:comment>Name of the secure tag, created with TagManager's TagValue API.
@pattern tagValues/[0-9]+</rdfs:comment>
    <rdfs:domain rdf:resource="http://example.org/onto/class/google_compute_region_network_firewall_policy_with_rules"/>
    <rdfs:range rdf:resource="http://www.w3.org/2001/XMLSchema#string"/>
  </owl:DatatypeProperty>
  <owl:DatatypeProperty rdf:about="http://example.org/onto/prop/google_compute_region_network_firewall_policy_with_rules_state">
    <rdfs:label>state</rdfs:label>
    <rdfs:comment>[Output Only] State of the secure tag, either 'EFFECTIVE' or
'INEFFECTIVE'. A secure tag is 'INEFFECTIVE' when it is deleted
or its network is deleted.</rdfs:comment>
    <rdfs:domain rdf:resource="http://example.org/onto/class/google_compute_region_network_firewall_policy_with_rules"/>
    <rdfs:range rdf:resource="http://www.w3.org/2001/XMLSchema#string"/>
  </owl:DatatypeProperty>
  <owl:DatatypeProperty rdf:about="http://example.org/onto/prop/google_compute_region_network_firewall_policy_with_rules_create">
    <rdfs:label>create</rdfs:label>
    <rdfs:domain rdf:resource="http://example.org/onto/class/google_compute_region_network_firewall_policy_with_rules"/>
    <rdfs:range rdf:resource="http://www.w3.org/2001/XMLSchema#string"/>
  </owl:DatatypeProperty>
  <owl:DatatypeProperty rdf:about="http://example.org/onto/prop/google_compute_region_network_firewall_policy_with_rules_delete">
    <rdfs:label>delete</rdfs:label>
    <rdfs:domain rdf:resource="http://example.org/onto/class/google_compute_region_network_firewall_policy_with_rules"/>
    <rdfs:range rdf:resource="http://www.w3.org/2001/XMLSchema#string"/>
  </owl:DatatypeProperty>
  <owl:DatatypeProperty rdf:about="http://example.org/onto/prop/google_compute_region_network_firewall_policy_with_rules_update">
    <rdfs:label>update</rdfs:label>
    <rdfs:domain rdf:resource="http://example.org/onto/class/google_compute_region_network_firewall_policy_with_rules"/>
    <rdfs:range rdf:resource="http://www.w3.org/2001/XMLSchema#string"/>
  </owl:DatatypeProperty>
</rdf:RDF>
