<?xml version="1.0" encoding="UTF-8"?>
<rdf:RDF
  xmlns:rdf="http://www.w3.org/1999/02/22-rdf-syntax-ns#"
  xmlns:rdfs="http://www.w3.org/2000/01/rdf-schema#"
  xmlns:owl="http://www.w3.org/2002/07/owl#"
  xmlns:xsd="http://www.w3.org/2001/XMLSchema#"
  xml:base="http://example.org/onto/">
  <owl:Class rdf:about="http://example.org/onto/class/google_netapp_storage_pool">
    <rdfs:label>google_netapp_storage_pool</rdfs:label>
    <rdfs:comment>#
#     ***     AUTO GENERATED CODE    ***    Type: MMv1     ***
#
# ----------------------------------------------------------------------------
#
#     This code is generated by Magic Modules using the following:
#
#     Configuration: https:#github.com/GoogleCloudPlatform/magic-modules/tree/main/mmv1/products/netapp/StoragePool.yaml
#     Template:      https:#github.com/GoogleCloudPlatform/magic-modules/tree/main/mmv1/templates/terraform/resource.html.markdown.tmpl
#
#     DO NOT EDIT this file directly. Any changes made to this file will be
#     overwritten during the next generation cycle.
#
# ----------------------------------------------------------------------------
subcategory: "Google Cloud NetApp Volumes"
description: |-
  Storage pools act as containers for volumes.
---</rdfs:comment>
  </owl:Class>
  <owl:DatatypeProperty rdf:about="http://example.org/onto/prop/google_netapp_storage_pool_active_directory">
    <rdfs:label>active_directory</rdfs:label>
    <rdfs:comment>Specifies the Active Directory policy to be used. Format: 'projects/{{project}}/locations/{{location}}/activeDirectories/{{name}}'.
The policy needs to be in the same location as the storage pool.</rdfs:comment>
    <rdfs:domain rdf:resource="http://example.org/onto/class/google_netapp_storage_pool"/>
    <rdfs:range rdf:resource="http://www.w3.org/2001/XMLSchema#string"/>
  </owl:DatatypeProperty>
  <owl:DatatypeProperty rdf:about="http://example.org/onto/prop/google_netapp_storage_pool_allow_auto_tiering">
    <rdfs:label>allow_auto_tiering</rdfs:label>
    <rdfs:comment>Optional. True if the storage pool supports Auto Tiering enabled volumes. Default is false.
Auto-tiering can be enabled after storage pool creation but it can't be disabled once enabled.</rdfs:comment>
    <rdfs:domain rdf:resource="http://example.org/onto/class/google_netapp_storage_pool"/>
    <rdfs:range rdf:resource="http://www.w3.org/2001/XMLSchema#string"/>
  </owl:DatatypeProperty>
  <owl:DatatypeProperty rdf:about="http://example.org/onto/prop/google_netapp_storage_pool_available_throughput_mibps">
    <rdfs:label>available_throughput_mibps</rdfs:label>
    <rdfs:comment>Available throughput of the storage pool (in MiB/s).</rdfs:comment>
    <rdfs:domain rdf:resource="http://example.org/onto/class/google_netapp_storage_pool"/>
    <rdfs:range rdf:resource="http://www.w3.org/2001/XMLSchema#string"/>
  </owl:DatatypeProperty>
  <owl:DatatypeProperty rdf:about="http://example.org/onto/prop/google_netapp_storage_pool_capacity_gib">
    <rdfs:label>capacity_gib</rdfs:label>
    <rdfs:comment>Capacity of the storage pool (in GiB).</rdfs:comment>
    <rdfs:domain rdf:resource="http://example.org/onto/class/google_netapp_storage_pool"/>
    <rdfs:range rdf:resource="http://www.w3.org/2001/XMLSchema#string"/>
  </owl:DatatypeProperty>
  <owl:DatatypeProperty rdf:about="http://example.org/onto/prop/google_netapp_storage_pool_cold_tier_size_used_gib">
    <rdfs:label>cold_tier_size_used_gib</rdfs:label>
    <rdfs:comment>Total cold tier data rounded down to the nearest GiB used by the storage pool.</rdfs:comment>
    <rdfs:domain rdf:resource="http://example.org/onto/class/google_netapp_storage_pool"/>
    <rdfs:range rdf:resource="http://www.w3.org/2001/XMLSchema#string"/>
  </owl:DatatypeProperty>
  <owl:DatatypeProperty rdf:about="http://example.org/onto/prop/google_netapp_storage_pool_custom_performance_enabled">
    <rdfs:label>custom_performance_enabled</rdfs:label>
    <rdfs:comment>Optional. True if using Independent Scaling of capacity and performance (Hyperdisk). Default is false.</rdfs:comment>
    <rdfs:domain rdf:resource="http://example.org/onto/class/google_netapp_storage_pool"/>
    <rdfs:range rdf:resource="http://www.w3.org/2001/XMLSchema#string"/>
  </owl:DatatypeProperty>
  <owl:DatatypeProperty rdf:about="http://example.org/onto/prop/google_netapp_storage_pool_description">
    <rdfs:label>description</rdfs:label>
    <rdfs:comment>An optional description of this resource.</rdfs:comment>
    <rdfs:domain rdf:resource="http://example.org/onto/class/google_netapp_storage_pool"/>
    <rdfs:range rdf:resource="http://www.w3.org/2001/XMLSchema#string"/>
  </owl:DatatypeProperty>
  <owl:DatatypeProperty rdf:about="http://example.org/onto/prop/google_netapp_storage_pool_effective_labels">
    <rdfs:label>effective_labels</rdfs:label>
    <rdfs:comment>All of labels (key/value pairs) present on the resource in GCP, including the labels configured through Terraform, other clients and services.</rdfs:comment>
    <rdfs:domain rdf:resource="http://example.org/onto/class/google_netapp_storage_pool"/>
    <rdfs:range rdf:resource="http://www.w3.org/2001/XMLSchema#string"/>
  </owl:DatatypeProperty>
  <owl:DatatypeProperty rdf:about="http://example.org/onto/prop/google_netapp_storage_pool_enable_hot_tier_auto_resize">
    <rdfs:label>enable_hot_tier_auto_resize</rdfs:label>
    <rdfs:comment>Flag indicating that the hot-tier threshold will be auto-increased by 10% of the hot-tier when it hits 100%. Default is true.
The increment will kick in only if the new size after increment is still less than or equal to storage pool size.</rdfs:comment>
    <rdfs:domain rdf:resource="http://example.org/onto/class/google_netapp_storage_pool"/>
    <rdfs:range rdf:resource="http://www.w3.org/2001/XMLSchema#string"/>
  </owl:DatatypeProperty>
  <owl:DatatypeProperty rdf:about="http://example.org/onto/prop/google_netapp_storage_pool_encryption_type">
    <rdfs:label>encryption_type</rdfs:label>
    <rdfs:comment>Reports if volumes in the pool are encrypted using a Google-managed encryption key or CMEK.</rdfs:comment>
    <rdfs:domain rdf:resource="http://example.org/onto/class/google_netapp_storage_pool"/>
    <rdfs:range rdf:resource="http://www.w3.org/2001/XMLSchema#string"/>
  </owl:DatatypeProperty>
  <owl:DatatypeProperty rdf:about="http://example.org/onto/prop/google_netapp_storage_pool_hot_tier_size_gib">
    <rdfs:label>hot_tier_size_gib</rdfs:label>
    <rdfs:comment>Total hot tier capacity for the Storage Pool. It is applicable only to Flex service level.
It should be less than the minimum storage pool size and cannot be more than the current storage pool size. It cannot be decreased once set.</rdfs:comment>
    <rdfs:domain rdf:resource="http://example.org/onto/class/google_netapp_storage_pool"/>
    <rdfs:range rdf:resource="http://www.w3.org/2001/XMLSchema#string"/>
  </owl:DatatypeProperty>
  <owl:DatatypeProperty rdf:about="http://example.org/onto/prop/google_netapp_storage_pool_hot_tier_size_used_gib">
    <rdfs:label>hot_tier_size_used_gib</rdfs:label>
    <rdfs:comment>Total hot tier data rounded down to the nearest GiB used by the storage pool.</rdfs:comment>
    <rdfs:domain rdf:resource="http://example.org/onto/class/google_netapp_storage_pool"/>
    <rdfs:range rdf:resource="http://www.w3.org/2001/XMLSchema#string"/>
  </owl:DatatypeProperty>
  <owl:DatatypeProperty rdf:about="http://example.org/onto/prop/google_netapp_storage_pool_id">
    <rdfs:label>id</rdfs:label>
    <rdfs:domain rdf:resource="http://example.org/onto/class/google_netapp_storage_pool"/>
    <rdfs:range rdf:resource="http://www.w3.org/2001/XMLSchema#string"/>
  </owl:DatatypeProperty>
  <owl:DatatypeProperty rdf:about="http://example.org/onto/prop/google_netapp_storage_pool_kms_config">
    <rdfs:label>kms_config</rdfs:label>
    <rdfs:comment>Specifies the CMEK policy to be used for volume encryption. Format: 'projects/{{project}}/locations/{{location}}/kmsConfigs/{{name}}'.
The policy needs to be in the same location as the storage pool.</rdfs:comment>
    <rdfs:domain rdf:resource="http://example.org/onto/class/google_netapp_storage_pool"/>
    <rdfs:range rdf:resource="http://www.w3.org/2001/XMLSchema#string"/>
  </owl:DatatypeProperty>
  <owl:DatatypeProperty rdf:about="http://example.org/onto/prop/google_netapp_storage_pool_labels">
    <rdfs:label>labels</rdfs:label>
    <rdfs:comment>Labels as key value pairs. Example: '{ "owner": "Bob", "department": "finance", "purpose": "testing" }'.


**Note**: This field is non-authoritative, and will only manage the labels present in your configuration.
Please refer to the field 'effective_labels' for all of the labels present on the resource.</rdfs:comment>
    <rdfs:domain rdf:resource="http://example.org/onto/class/google_netapp_storage_pool"/>
    <rdfs:range rdf:resource="http://www.w3.org/2001/XMLSchema#string"/>
  </owl:DatatypeProperty>
  <owl:DatatypeProperty rdf:about="http://example.org/onto/prop/google_netapp_storage_pool_ldap_enabled">
    <rdfs:label>ldap_enabled</rdfs:label>
    <rdfs:comment>When enabled, the volumes uses Active Directory as LDAP name service for UID/GID lookups. Required to enable extended group support for NFSv3,
using security identifiers for NFSv4.1 or principal names for kerberized NFSv4.1.</rdfs:comment>
    <rdfs:domain rdf:resource="http://example.org/onto/class/google_netapp_storage_pool"/>
    <rdfs:range rdf:resource="http://www.w3.org/2001/XMLSchema#string"/>
  </owl:DatatypeProperty>
  <owl:DatatypeProperty rdf:about="http://example.org/onto/prop/google_netapp_storage_pool_location">
    <rdfs:label>location</rdfs:label>
    <rdfs:comment>Name of the location. For zonal Flex pools specify a zone name, in all other cases a region name.</rdfs:comment>
    <rdfs:domain rdf:resource="http://example.org/onto/class/google_netapp_storage_pool"/>
    <rdfs:range rdf:resource="http://www.w3.org/2001/XMLSchema#string"/>
  </owl:DatatypeProperty>
  <owl:DatatypeProperty rdf:about="http://example.org/onto/prop/google_netapp_storage_pool_name">
    <rdfs:label>name</rdfs:label>
    <rdfs:comment>The resource name of the storage pool. Needs to be unique per location/region.</rdfs:comment>
    <rdfs:domain rdf:resource="http://example.org/onto/class/google_netapp_storage_pool"/>
    <rdfs:range rdf:resource="http://www.w3.org/2001/XMLSchema#string"/>
  </owl:DatatypeProperty>
  <owl:DatatypeProperty rdf:about="http://example.org/onto/prop/google_netapp_storage_pool_network">
    <rdfs:label>network</rdfs:label>
    <rdfs:comment>VPC network name with format: 'projects/{{project}}/global/networks/{{network}}'</rdfs:comment>
    <rdfs:domain rdf:resource="http://example.org/onto/class/google_netapp_storage_pool"/>
    <rdfs:range rdf:resource="http://www.w3.org/2001/XMLSchema#string"/>
  </owl:DatatypeProperty>
  <owl:DatatypeProperty rdf:about="http://example.org/onto/prop/google_netapp_storage_pool_project">
    <rdfs:label>project</rdfs:label>
    <rdfs:domain rdf:resource="http://example.org/onto/class/google_netapp_storage_pool"/>
    <rdfs:range rdf:resource="http://www.w3.org/2001/XMLSchema#string"/>
  </owl:DatatypeProperty>
  <owl:DatatypeProperty rdf:about="http://example.org/onto/prop/google_netapp_storage_pool_qos_type">
    <rdfs:label>qos_type</rdfs:label>
    <rdfs:comment>QoS (Quality of Service) type of the storage pool.
Possible values are: AUTO, MANUAL. Possible values: ["QOS_TYPE_UNSPECIFIED", "AUTO", "MANUAL"]</rdfs:comment>
    <rdfs:domain rdf:resource="http://example.org/onto/class/google_netapp_storage_pool"/>
    <rdfs:range rdf:resource="http://www.w3.org/2001/XMLSchema#string"/>
  </owl:DatatypeProperty>
  <owl:DatatypeProperty rdf:about="http://example.org/onto/prop/google_netapp_storage_pool_replica_zone">
    <rdfs:label>replica_zone</rdfs:label>
    <rdfs:comment>Specifies the replica zone for regional Flex pools. 'zone' and 'replica_zone' values can be swapped to initiate a
[zone switch](https://cloud.google.com/netapp/volumes/docs/configure-and-use/storage-pools/edit-or-delete-storage-pool#switch_active_and_replica_zones).</rdfs:comment>
    <rdfs:domain rdf:resource="http://example.org/onto/class/google_netapp_storage_pool"/>
    <rdfs:range rdf:resource="http://www.w3.org/2001/XMLSchema#string"/>
  </owl:DatatypeProperty>
  <owl:DatatypeProperty rdf:about="http://example.org/onto/prop/google_netapp_storage_pool_service_level">
    <rdfs:label>service_level</rdfs:label>
    <rdfs:comment>Service level of the storage pool. Possible values: ["PREMIUM", "EXTREME", "STANDARD", "FLEX"]</rdfs:comment>
    <rdfs:domain rdf:resource="http://example.org/onto/class/google_netapp_storage_pool"/>
    <rdfs:range rdf:resource="http://www.w3.org/2001/XMLSchema#string"/>
  </owl:DatatypeProperty>
  <owl:DatatypeProperty rdf:about="http://example.org/onto/prop/google_netapp_storage_pool_terraform_labels">
    <rdfs:label>terraform_labels</rdfs:label>
    <rdfs:comment>The combination of labels configured directly on the resource
 and default labels configured on the provider.</rdfs:comment>
    <rdfs:domain rdf:resource="http://example.org/onto/class/google_netapp_storage_pool"/>
    <rdfs:range rdf:resource="http://www.w3.org/2001/XMLSchema#string"/>
  </owl:DatatypeProperty>
  <owl:DatatypeProperty rdf:about="http://example.org/onto/prop/google_netapp_storage_pool_total_iops">
    <rdfs:label>total_iops</rdfs:label>
    <rdfs:comment>Optional. Custom Performance Total IOPS of the pool If not provided, it will be calculated based on the totalThroughputMibps</rdfs:comment>
    <rdfs:domain rdf:resource="http://example.org/onto/class/google_netapp_storage_pool"/>
    <rdfs:range rdf:resource="http://www.w3.org/2001/XMLSchema#string"/>
  </owl:DatatypeProperty>
  <owl:DatatypeProperty rdf:about="http://example.org/onto/prop/google_netapp_storage_pool_total_throughput_mibps">
    <rdfs:label>total_throughput_mibps</rdfs:label>
    <rdfs:comment>Optional. Custom Performance Total Throughput of the pool (in MiB/s).</rdfs:comment>
    <rdfs:domain rdf:resource="http://example.org/onto/class/google_netapp_storage_pool"/>
    <rdfs:range rdf:resource="http://www.w3.org/2001/XMLSchema#string"/>
  </owl:DatatypeProperty>
  <owl:DatatypeProperty rdf:about="http://example.org/onto/prop/google_netapp_storage_pool_volume_capacity_gib">
    <rdfs:label>volume_capacity_gib</rdfs:label>
    <rdfs:comment>Size allocated to volumes in the storage pool (in GiB).</rdfs:comment>
    <rdfs:domain rdf:resource="http://example.org/onto/class/google_netapp_storage_pool"/>
    <rdfs:range rdf:resource="http://www.w3.org/2001/XMLSchema#string"/>
  </owl:DatatypeProperty>
  <owl:DatatypeProperty rdf:about="http://example.org/onto/prop/google_netapp_storage_pool_volume_count">
    <rdfs:label>volume_count</rdfs:label>
    <rdfs:comment>Number of volume in the storage pool.</rdfs:comment>
    <rdfs:domain rdf:resource="http://example.org/onto/class/google_netapp_storage_pool"/>
    <rdfs:range rdf:resource="http://www.w3.org/2001/XMLSchema#string"/>
  </owl:DatatypeProperty>
  <owl:DatatypeProperty rdf:about="http://example.org/onto/prop/google_netapp_storage_pool_zone">
    <rdfs:label>zone</rdfs:label>
    <rdfs:comment>Specifies the active zone for regional Flex pools. 'zone' and 'replica_zone' values can be swapped to initiate a
[zone switch](https://cloud.google.com/netapp/volumes/docs/configure-and-use/storage-pools/edit-or-delete-storage-pool#switch_active_and_replica_zones).
If you want to create a zonal Flex pool, specify a zone name for 'location' and omit 'zone'.</rdfs:comment>
    <rdfs:domain rdf:resource="http://example.org/onto/class/google_netapp_storage_pool"/>
    <rdfs:range rdf:resource="http://www.w3.org/2001/XMLSchema#string"/>
  </owl:DatatypeProperty>
  <owl:DatatypeProperty rdf:about="http://example.org/onto/prop/google_netapp_storage_pool_create">
    <rdfs:label>create</rdfs:label>
    <rdfs:domain rdf:resource="http://example.org/onto/class/google_netapp_storage_pool"/>
    <rdfs:range rdf:resource="http://www.w3.org/2001/XMLSchema#string"/>
  </owl:DatatypeProperty>
  <owl:DatatypeProperty rdf:about="http://example.org/onto/prop/google_netapp_storage_pool_delete">
    <rdfs:label>delete</rdfs:label>
    <rdfs:domain rdf:resource="http://example.org/onto/class/google_netapp_storage_pool"/>
    <rdfs:range rdf:resource="http://www.w3.org/2001/XMLSchema#string"/>
  </owl:DatatypeProperty>
  <owl:DatatypeProperty rdf:about="http://example.org/onto/prop/google_netapp_storage_pool_update">
    <rdfs:label>update</rdfs:label>
    <rdfs:domain rdf:resource="http://example.org/onto/class/google_netapp_storage_pool"/>
    <rdfs:range rdf:resource="http://www.w3.org/2001/XMLSchema#string"/>
  </owl:DatatypeProperty>
</rdf:RDF>
