<?xml version="1.0" encoding="UTF-8"?>
<rdf:RDF
  xmlns:rdf="http://www.w3.org/1999/02/22-rdf-syntax-ns#"
  xmlns:rdfs="http://www.w3.org/2000/01/rdf-schema#"
  xmlns:owl="http://www.w3.org/2002/07/owl#"
  xmlns:xsd="http://www.w3.org/2001/XMLSchema#"
  xml:base="http://example.org/onto/">
  <owl:Class rdf:about="http://example.org/onto/class/google_cloudfunctions_function">
    <rdfs:label>google_cloudfunctions_function</rdfs:label>
    <rdfs:comment>#
#     ***     AUTO GENERATED CODE    ***    Type: Handwritten     ***
#
# ----------------------------------------------------------------------------
#
#     This code is generated by Magic Modules using the following:
#
#     Source file: https://github.com/GoogleCloudPlatform/magic-modules/tree/main/mmv1/third_party/terraform/website/docs/r/cloudfunctions_function.html.markdown
#
#     DO NOT EDIT this file directly. Any changes made to this file will be
#     overwritten during the next generation cycle.
#
# ----------------------------------------------------------------------------
subcategory: "Cloud Functions"
description: |-
  Creates a new Cloud Function.
---</rdfs:comment>
  </owl:Class>
  <owl:DatatypeProperty rdf:about="http://example.org/onto/prop/google_cloudfunctions_function_available_memory_mb">
    <rdfs:label>available_memory_mb</rdfs:label>
    <rdfs:comment>Memory (in MB), available to the function. Default value is 256. Possible values include 128, 256, 512, 1024, etc.</rdfs:comment>
    <rdfs:domain rdf:resource="http://example.org/onto/class/google_cloudfunctions_function"/>
    <rdfs:range rdf:resource="http://www.w3.org/2001/XMLSchema#string"/>
  </owl:DatatypeProperty>
  <owl:DatatypeProperty rdf:about="http://example.org/onto/prop/google_cloudfunctions_function_build_environment_variables">
    <rdfs:label>build_environment_variables</rdfs:label>
    <rdfs:comment>A set of key/value environment variable pairs available during build time.</rdfs:comment>
    <rdfs:domain rdf:resource="http://example.org/onto/class/google_cloudfunctions_function"/>
    <rdfs:range rdf:resource="http://www.w3.org/2001/XMLSchema#string"/>
  </owl:DatatypeProperty>
  <owl:DatatypeProperty rdf:about="http://example.org/onto/prop/google_cloudfunctions_function_build_service_account">
    <rdfs:label>build_service_account</rdfs:label>
    <rdfs:comment>The fully-qualified name of the service account to be used for the build step of deploying this function</rdfs:comment>
    <rdfs:domain rdf:resource="http://example.org/onto/class/google_cloudfunctions_function"/>
    <rdfs:range rdf:resource="http://www.w3.org/2001/XMLSchema#string"/>
  </owl:DatatypeProperty>
  <owl:DatatypeProperty rdf:about="http://example.org/onto/prop/google_cloudfunctions_function_build_worker_pool">
    <rdfs:label>build_worker_pool</rdfs:label>
    <rdfs:comment>Name of the Cloud Build Custom Worker Pool that should be used to build the function.</rdfs:comment>
    <rdfs:domain rdf:resource="http://example.org/onto/class/google_cloudfunctions_function"/>
    <rdfs:range rdf:resource="http://www.w3.org/2001/XMLSchema#string"/>
  </owl:DatatypeProperty>
  <owl:DatatypeProperty rdf:about="http://example.org/onto/prop/google_cloudfunctions_function_description">
    <rdfs:label>description</rdfs:label>
    <rdfs:comment>Description of the function.</rdfs:comment>
    <rdfs:domain rdf:resource="http://example.org/onto/class/google_cloudfunctions_function"/>
    <rdfs:range rdf:resource="http://www.w3.org/2001/XMLSchema#string"/>
  </owl:DatatypeProperty>
  <owl:DatatypeProperty rdf:about="http://example.org/onto/prop/google_cloudfunctions_function_docker_registry">
    <rdfs:label>docker_registry</rdfs:label>
    <rdfs:comment>Docker Registry to use for storing the function's Docker images. Allowed values are ARTIFACT_REGISTRY (default) and CONTAINER_REGISTRY.</rdfs:comment>
    <rdfs:domain rdf:resource="http://example.org/onto/class/google_cloudfunctions_function"/>
    <rdfs:range rdf:resource="http://www.w3.org/2001/XMLSchema#string"/>
  </owl:DatatypeProperty>
  <owl:DatatypeProperty rdf:about="http://example.org/onto/prop/google_cloudfunctions_function_docker_repository">
    <rdfs:label>docker_repository</rdfs:label>
    <rdfs:comment>User managed repository created in Artifact Registry optionally with a customer managed encryption key. If specified, deployments will use Artifact Registry for storing images built with Cloud Build.</rdfs:comment>
    <rdfs:domain rdf:resource="http://example.org/onto/class/google_cloudfunctions_function"/>
    <rdfs:range rdf:resource="http://www.w3.org/2001/XMLSchema#string"/>
  </owl:DatatypeProperty>
  <owl:DatatypeProperty rdf:about="http://example.org/onto/prop/google_cloudfunctions_function_effective_labels">
    <rdfs:label>effective_labels</rdfs:label>
    <rdfs:comment>All of labels (key/value pairs) present on the resource in GCP, including the labels configured through Terraform, other clients and services.</rdfs:comment>
    <rdfs:domain rdf:resource="http://example.org/onto/class/google_cloudfunctions_function"/>
    <rdfs:range rdf:resource="http://www.w3.org/2001/XMLSchema#string"/>
  </owl:DatatypeProperty>
  <owl:DatatypeProperty rdf:about="http://example.org/onto/prop/google_cloudfunctions_function_entry_point">
    <rdfs:label>entry_point</rdfs:label>
    <rdfs:comment>Name of the function that will be executed when the Google Cloud Function is triggered.</rdfs:comment>
    <rdfs:domain rdf:resource="http://example.org/onto/class/google_cloudfunctions_function"/>
    <rdfs:range rdf:resource="http://www.w3.org/2001/XMLSchema#string"/>
  </owl:DatatypeProperty>
  <owl:DatatypeProperty rdf:about="http://example.org/onto/prop/google_cloudfunctions_function_environment_variables">
    <rdfs:label>environment_variables</rdfs:label>
    <rdfs:comment>A set of key/value environment variable pairs to assign to the function.</rdfs:comment>
    <rdfs:domain rdf:resource="http://example.org/onto/class/google_cloudfunctions_function"/>
    <rdfs:range rdf:resource="http://www.w3.org/2001/XMLSchema#string"/>
  </owl:DatatypeProperty>
  <owl:DatatypeProperty rdf:about="http://example.org/onto/prop/google_cloudfunctions_function_https_trigger_security_level">
    <rdfs:label>https_trigger_security_level</rdfs:label>
    <rdfs:comment>The security level for the function. Defaults to SECURE_OPTIONAL. Valid only if trigger_http is used.</rdfs:comment>
    <rdfs:domain rdf:resource="http://example.org/onto/class/google_cloudfunctions_function"/>
    <rdfs:range rdf:resource="http://www.w3.org/2001/XMLSchema#string"/>
  </owl:DatatypeProperty>
  <owl:DatatypeProperty rdf:about="http://example.org/onto/prop/google_cloudfunctions_function_https_trigger_url">
    <rdfs:label>https_trigger_url</rdfs:label>
    <rdfs:comment>URL which triggers function execution. Returned only if trigger_http is used.</rdfs:comment>
    <rdfs:domain rdf:resource="http://example.org/onto/class/google_cloudfunctions_function"/>
    <rdfs:range rdf:resource="http://www.w3.org/2001/XMLSchema#string"/>
  </owl:DatatypeProperty>
  <owl:DatatypeProperty rdf:about="http://example.org/onto/prop/google_cloudfunctions_function_id">
    <rdfs:label>id</rdfs:label>
    <rdfs:domain rdf:resource="http://example.org/onto/class/google_cloudfunctions_function"/>
    <rdfs:range rdf:resource="http://www.w3.org/2001/XMLSchema#string"/>
  </owl:DatatypeProperty>
  <owl:DatatypeProperty rdf:about="http://example.org/onto/prop/google_cloudfunctions_function_ingress_settings">
    <rdfs:label>ingress_settings</rdfs:label>
    <rdfs:comment>String value that controls what traffic can reach the function. Allowed values are ALLOW_ALL and ALLOW_INTERNAL_ONLY. Changes to this field will recreate the cloud function.</rdfs:comment>
    <rdfs:domain rdf:resource="http://example.org/onto/class/google_cloudfunctions_function"/>
    <rdfs:range rdf:resource="http://www.w3.org/2001/XMLSchema#string"/>
  </owl:DatatypeProperty>
  <owl:DatatypeProperty rdf:about="http://example.org/onto/prop/google_cloudfunctions_function_kms_key_name">
    <rdfs:label>kms_key_name</rdfs:label>
    <rdfs:comment>Resource name of a KMS crypto key (managed by the user) used to encrypt/decrypt function resources.</rdfs:comment>
    <rdfs:domain rdf:resource="http://example.org/onto/class/google_cloudfunctions_function"/>
    <rdfs:range rdf:resource="http://www.w3.org/2001/XMLSchema#string"/>
  </owl:DatatypeProperty>
  <owl:DatatypeProperty rdf:about="http://example.org/onto/prop/google_cloudfunctions_function_labels">
    <rdfs:label>labels</rdfs:label>
    <rdfs:comment>A set of key/value label pairs to assign to the function. Label keys must follow the requirements at https://cloud.google.com/resource-manager/docs/creating-managing-labels#requirements.

				**Note**: This field is non-authoritative, and will only manage the labels present in your configuration.
				Please refer to the field 'effective_labels' for all of the labels present on the resource.</rdfs:comment>
    <rdfs:domain rdf:resource="http://example.org/onto/class/google_cloudfunctions_function"/>
    <rdfs:range rdf:resource="http://www.w3.org/2001/XMLSchema#string"/>
  </owl:DatatypeProperty>
  <owl:DatatypeProperty rdf:about="http://example.org/onto/prop/google_cloudfunctions_function_max_instances">
    <rdfs:label>max_instances</rdfs:label>
    <rdfs:comment>The limit on the maximum number of function instances that may coexist at a given time.</rdfs:comment>
    <rdfs:domain rdf:resource="http://example.org/onto/class/google_cloudfunctions_function"/>
    <rdfs:range rdf:resource="http://www.w3.org/2001/XMLSchema#string"/>
  </owl:DatatypeProperty>
  <owl:DatatypeProperty rdf:about="http://example.org/onto/prop/google_cloudfunctions_function_min_instances">
    <rdfs:label>min_instances</rdfs:label>
    <rdfs:comment>The limit on the minimum number of function instances that may coexist at a given time.</rdfs:comment>
    <rdfs:domain rdf:resource="http://example.org/onto/class/google_cloudfunctions_function"/>
    <rdfs:range rdf:resource="http://www.w3.org/2001/XMLSchema#string"/>
  </owl:DatatypeProperty>
  <owl:DatatypeProperty rdf:about="http://example.org/onto/prop/google_cloudfunctions_function_name">
    <rdfs:label>name</rdfs:label>
    <rdfs:comment>A user-defined name of the function. Function names must be unique globally.</rdfs:comment>
    <rdfs:domain rdf:resource="http://example.org/onto/class/google_cloudfunctions_function"/>
    <rdfs:range rdf:resource="http://www.w3.org/2001/XMLSchema#string"/>
  </owl:DatatypeProperty>
  <owl:DatatypeProperty rdf:about="http://example.org/onto/prop/google_cloudfunctions_function_project">
    <rdfs:label>project</rdfs:label>
    <rdfs:comment>Project of the function. If it is not provided, the provider project is used.</rdfs:comment>
    <rdfs:domain rdf:resource="http://example.org/onto/class/google_cloudfunctions_function"/>
    <rdfs:range rdf:resource="http://www.w3.org/2001/XMLSchema#string"/>
  </owl:DatatypeProperty>
  <owl:DatatypeProperty rdf:about="http://example.org/onto/prop/google_cloudfunctions_function_region">
    <rdfs:label>region</rdfs:label>
    <rdfs:comment>Region of function. If it is not provided, the provider region is used.</rdfs:comment>
    <rdfs:domain rdf:resource="http://example.org/onto/class/google_cloudfunctions_function"/>
    <rdfs:range rdf:resource="http://www.w3.org/2001/XMLSchema#string"/>
  </owl:DatatypeProperty>
  <owl:DatatypeProperty rdf:about="http://example.org/onto/prop/google_cloudfunctions_function_runtime">
    <rdfs:label>runtime</rdfs:label>
    <rdfs:comment>The runtime in which the function is going to run. Eg. "nodejs20", "python37", "go111".</rdfs:comment>
    <rdfs:domain rdf:resource="http://example.org/onto/class/google_cloudfunctions_function"/>
    <rdfs:range rdf:resource="http://www.w3.org/2001/XMLSchema#string"/>
  </owl:DatatypeProperty>
  <owl:DatatypeProperty rdf:about="http://example.org/onto/prop/google_cloudfunctions_function_service_account_email">
    <rdfs:label>service_account_email</rdfs:label>
    <rdfs:comment>If provided, the self-provided service account to run the function with.</rdfs:comment>
    <rdfs:domain rdf:resource="http://example.org/onto/class/google_cloudfunctions_function"/>
    <rdfs:range rdf:resource="http://www.w3.org/2001/XMLSchema#string"/>
  </owl:DatatypeProperty>
  <owl:DatatypeProperty rdf:about="http://example.org/onto/prop/google_cloudfunctions_function_source_archive_bucket">
    <rdfs:label>source_archive_bucket</rdfs:label>
    <rdfs:comment>The GCS bucket containing the zip archive which contains the function.</rdfs:comment>
    <rdfs:domain rdf:resource="http://example.org/onto/class/google_cloudfunctions_function"/>
    <rdfs:range rdf:resource="http://www.w3.org/2001/XMLSchema#string"/>
  </owl:DatatypeProperty>
  <owl:DatatypeProperty rdf:about="http://example.org/onto/prop/google_cloudfunctions_function_source_archive_object">
    <rdfs:label>source_archive_object</rdfs:label>
    <rdfs:comment>The source archive object (file) in archive bucket.</rdfs:comment>
    <rdfs:domain rdf:resource="http://example.org/onto/class/google_cloudfunctions_function"/>
    <rdfs:range rdf:resource="http://www.w3.org/2001/XMLSchema#string"/>
  </owl:DatatypeProperty>
  <owl:DatatypeProperty rdf:about="http://example.org/onto/prop/google_cloudfunctions_function_status">
    <rdfs:label>status</rdfs:label>
    <rdfs:comment>Describes the current stage of a deployment.</rdfs:comment>
    <rdfs:domain rdf:resource="http://example.org/onto/class/google_cloudfunctions_function"/>
    <rdfs:range rdf:resource="http://www.w3.org/2001/XMLSchema#string"/>
  </owl:DatatypeProperty>
  <owl:DatatypeProperty rdf:about="http://example.org/onto/prop/google_cloudfunctions_function_terraform_labels">
    <rdfs:label>terraform_labels</rdfs:label>
    <rdfs:comment>The combination of labels configured directly on the resource and default labels configured on the provider.</rdfs:comment>
    <rdfs:domain rdf:resource="http://example.org/onto/class/google_cloudfunctions_function"/>
    <rdfs:range rdf:resource="http://www.w3.org/2001/XMLSchema#string"/>
  </owl:DatatypeProperty>
  <owl:DatatypeProperty rdf:about="http://example.org/onto/prop/google_cloudfunctions_function_timeout">
    <rdfs:label>timeout</rdfs:label>
    <rdfs:comment>Timeout (in seconds) for the function. Default value is 60 seconds. Cannot be more than 540 seconds.</rdfs:comment>
    <rdfs:domain rdf:resource="http://example.org/onto/class/google_cloudfunctions_function"/>
    <rdfs:range rdf:resource="http://www.w3.org/2001/XMLSchema#string"/>
  </owl:DatatypeProperty>
  <owl:DatatypeProperty rdf:about="http://example.org/onto/prop/google_cloudfunctions_function_trigger_http">
    <rdfs:label>trigger_http</rdfs:label>
    <rdfs:comment>Boolean variable. Any HTTP request (of a supported type) to the endpoint will trigger function execution. Supported HTTP request types are: POST, PUT, GET, DELETE, and OPTIONS. Endpoint is returned as https_trigger_url. Cannot be used with trigger_bucket and trigger_topic.</rdfs:comment>
    <rdfs:domain rdf:resource="http://example.org/onto/class/google_cloudfunctions_function"/>
    <rdfs:range rdf:resource="http://www.w3.org/2001/XMLSchema#string"/>
  </owl:DatatypeProperty>
  <owl:DatatypeProperty rdf:about="http://example.org/onto/prop/google_cloudfunctions_function_version_id">
    <rdfs:label>version_id</rdfs:label>
    <rdfs:comment>The version identifier of the Cloud Function. Each deployment attempt results in a new version of a function being created.</rdfs:comment>
    <rdfs:domain rdf:resource="http://example.org/onto/class/google_cloudfunctions_function"/>
    <rdfs:range rdf:resource="http://www.w3.org/2001/XMLSchema#string"/>
  </owl:DatatypeProperty>
  <owl:DatatypeProperty rdf:about="http://example.org/onto/prop/google_cloudfunctions_function_vpc_connector">
    <rdfs:label>vpc_connector</rdfs:label>
    <rdfs:comment>The VPC Network Connector that this cloud function can connect to. It can be either the fully-qualified URI, or the short name of the network connector resource. The format of this field is projects/*/locations/*/connectors/*.</rdfs:comment>
    <rdfs:domain rdf:resource="http://example.org/onto/class/google_cloudfunctions_function"/>
    <rdfs:range rdf:resource="http://www.w3.org/2001/XMLSchema#string"/>
  </owl:DatatypeProperty>
  <owl:DatatypeProperty rdf:about="http://example.org/onto/prop/google_cloudfunctions_function_vpc_connector_egress_settings">
    <rdfs:label>vpc_connector_egress_settings</rdfs:label>
    <rdfs:comment>The egress settings for the connector, controlling what traffic is diverted through it. Allowed values are ALL_TRAFFIC and PRIVATE_RANGES_ONLY. Defaults to PRIVATE_RANGES_ONLY. If unset, this field preserves the previously set value.</rdfs:comment>
    <rdfs:domain rdf:resource="http://example.org/onto/class/google_cloudfunctions_function"/>
    <rdfs:range rdf:resource="http://www.w3.org/2001/XMLSchema#string"/>
  </owl:DatatypeProperty>
  <owl:DatatypeProperty rdf:about="http://example.org/onto/prop/google_cloudfunctions_function_event_type">
    <rdfs:label>event_type</rdfs:label>
    <rdfs:comment>The type of event to observe. For example: "google.storage.object.finalize". See the documentation on calling Cloud Functions for a full reference of accepted triggers.</rdfs:comment>
    <rdfs:domain rdf:resource="http://example.org/onto/class/google_cloudfunctions_function"/>
    <rdfs:range rdf:resource="http://www.w3.org/2001/XMLSchema#string"/>
  </owl:DatatypeProperty>
  <owl:DatatypeProperty rdf:about="http://example.org/onto/prop/google_cloudfunctions_function_resource">
    <rdfs:label>resource</rdfs:label>
    <rdfs:comment>The name or partial URI of the resource from which to observe events. For example, "myBucket" or "projects/my-project/topics/my-topic"</rdfs:comment>
    <rdfs:domain rdf:resource="http://example.org/onto/class/google_cloudfunctions_function"/>
    <rdfs:range rdf:resource="http://www.w3.org/2001/XMLSchema#string"/>
  </owl:DatatypeProperty>
  <owl:DatatypeProperty rdf:about="http://example.org/onto/prop/google_cloudfunctions_function_retry">
    <rdfs:label>retry</rdfs:label>
    <rdfs:comment>Whether the function should be retried on failure. Defaults to false.</rdfs:comment>
    <rdfs:domain rdf:resource="http://example.org/onto/class/google_cloudfunctions_function"/>
    <rdfs:range rdf:resource="http://www.w3.org/2001/XMLSchema#string"/>
  </owl:DatatypeProperty>
  <owl:DatatypeProperty rdf:about="http://example.org/onto/prop/google_cloudfunctions_function_runtime_version">
    <rdfs:label>runtime_version</rdfs:label>
    <rdfs:comment>The runtime version which was used during latest function deployment.</rdfs:comment>
    <rdfs:domain rdf:resource="http://example.org/onto/class/google_cloudfunctions_function"/>
    <rdfs:range rdf:resource="http://www.w3.org/2001/XMLSchema#string"/>
  </owl:DatatypeProperty>
  <owl:DatatypeProperty rdf:about="http://example.org/onto/prop/google_cloudfunctions_function_key">
    <rdfs:label>key</rdfs:label>
    <rdfs:comment>Name of the environment variable.</rdfs:comment>
    <rdfs:domain rdf:resource="http://example.org/onto/class/google_cloudfunctions_function"/>
    <rdfs:range rdf:resource="http://www.w3.org/2001/XMLSchema#string"/>
  </owl:DatatypeProperty>
  <owl:DatatypeProperty rdf:about="http://example.org/onto/prop/google_cloudfunctions_function_project_id">
    <rdfs:label>project_id</rdfs:label>
    <rdfs:comment>Project identifier (due to a known limitation, only project number is supported by this field) of the project that contains the secret. If not set, it will be populated with the function's project, assuming that the secret exists in the same project as of the function.</rdfs:comment>
    <rdfs:domain rdf:resource="http://example.org/onto/class/google_cloudfunctions_function"/>
    <rdfs:range rdf:resource="http://www.w3.org/2001/XMLSchema#string"/>
  </owl:DatatypeProperty>
  <owl:DatatypeProperty rdf:about="http://example.org/onto/prop/google_cloudfunctions_function_secret">
    <rdfs:label>secret</rdfs:label>
    <rdfs:comment>ID of the secret in secret manager (not the full resource name).</rdfs:comment>
    <rdfs:domain rdf:resource="http://example.org/onto/class/google_cloudfunctions_function"/>
    <rdfs:range rdf:resource="http://www.w3.org/2001/XMLSchema#string"/>
  </owl:DatatypeProperty>
  <owl:DatatypeProperty rdf:about="http://example.org/onto/prop/google_cloudfunctions_function_version">
    <rdfs:label>version</rdfs:label>
    <rdfs:comment>Version of the secret (version number or the string "latest"). It is recommended to use a numeric version for secret environment variables as any updates to the secret value is not reflected until new clones start.</rdfs:comment>
    <rdfs:domain rdf:resource="http://example.org/onto/class/google_cloudfunctions_function"/>
    <rdfs:range rdf:resource="http://www.w3.org/2001/XMLSchema#string"/>
  </owl:DatatypeProperty>
  <owl:DatatypeProperty rdf:about="http://example.org/onto/prop/google_cloudfunctions_function_mount_path">
    <rdfs:label>mount_path</rdfs:label>
    <rdfs:comment>The path within the container to mount the secret volume. For example, setting the mount_path as "/etc/secrets" would mount the secret value files under the "/etc/secrets" directory. This directory will also be completely shadowed and unavailable to mount any other secrets. Recommended mount paths: "/etc/secrets" Restricted mount paths: "/cloudsql", "/dev/log", "/pod", "/proc", "/var/log".</rdfs:comment>
    <rdfs:domain rdf:resource="http://example.org/onto/class/google_cloudfunctions_function"/>
    <rdfs:range rdf:resource="http://www.w3.org/2001/XMLSchema#string"/>
  </owl:DatatypeProperty>
  <owl:DatatypeProperty rdf:about="http://example.org/onto/prop/google_cloudfunctions_function_project_id">
    <rdfs:label>project_id</rdfs:label>
    <rdfs:comment>Project identifier (due to a known limitation, only project number is supported by this field) of the project that contains the secret. If not set, it will be populated with the function's project, assuming that the secret exists in the same project as of the function.</rdfs:comment>
    <rdfs:domain rdf:resource="http://example.org/onto/class/google_cloudfunctions_function"/>
    <rdfs:range rdf:resource="http://www.w3.org/2001/XMLSchema#string"/>
  </owl:DatatypeProperty>
  <owl:DatatypeProperty rdf:about="http://example.org/onto/prop/google_cloudfunctions_function_secret">
    <rdfs:label>secret</rdfs:label>
    <rdfs:comment>ID of the secret in secret manager (not the full resource name).</rdfs:comment>
    <rdfs:domain rdf:resource="http://example.org/onto/class/google_cloudfunctions_function"/>
    <rdfs:range rdf:resource="http://www.w3.org/2001/XMLSchema#string"/>
  </owl:DatatypeProperty>
  <owl:DatatypeProperty rdf:about="http://example.org/onto/prop/google_cloudfunctions_function_path">
    <rdfs:label>path</rdfs:label>
    <rdfs:comment>Relative path of the file under the mount path where the secret value for this version will be fetched and made available. For example, setting the mount_path as "/etc/secrets" and path as "/secret_foo" would mount the secret value file at "/etc/secrets/secret_foo".</rdfs:comment>
    <rdfs:domain rdf:resource="http://example.org/onto/class/google_cloudfunctions_function"/>
    <rdfs:range rdf:resource="http://www.w3.org/2001/XMLSchema#string"/>
  </owl:DatatypeProperty>
  <owl:DatatypeProperty rdf:about="http://example.org/onto/prop/google_cloudfunctions_function_version">
    <rdfs:label>version</rdfs:label>
    <rdfs:comment>Version of the secret (version number or the string "latest"). It is preferable to use "latest" version with secret volumes as secret value changes are reflected immediately.</rdfs:comment>
    <rdfs:domain rdf:resource="http://example.org/onto/class/google_cloudfunctions_function"/>
    <rdfs:range rdf:resource="http://www.w3.org/2001/XMLSchema#string"/>
  </owl:DatatypeProperty>
  <owl:DatatypeProperty rdf:about="http://example.org/onto/prop/google_cloudfunctions_function_deployed_url">
    <rdfs:label>deployed_url</rdfs:label>
    <rdfs:comment>The URL pointing to the hosted repository where the function was defined at the time of deployment.</rdfs:comment>
    <rdfs:domain rdf:resource="http://example.org/onto/class/google_cloudfunctions_function"/>
    <rdfs:range rdf:resource="http://www.w3.org/2001/XMLSchema#string"/>
  </owl:DatatypeProperty>
  <owl:DatatypeProperty rdf:about="http://example.org/onto/prop/google_cloudfunctions_function_url">
    <rdfs:label>url</rdfs:label>
    <rdfs:comment>The URL pointing to the hosted repository where the function is defined.</rdfs:comment>
    <rdfs:domain rdf:resource="http://example.org/onto/class/google_cloudfunctions_function"/>
    <rdfs:range rdf:resource="http://www.w3.org/2001/XMLSchema#string"/>
  </owl:DatatypeProperty>
  <owl:DatatypeProperty rdf:about="http://example.org/onto/prop/google_cloudfunctions_function_create">
    <rdfs:label>create</rdfs:label>
    <rdfs:domain rdf:resource="http://example.org/onto/class/google_cloudfunctions_function"/>
    <rdfs:range rdf:resource="http://www.w3.org/2001/XMLSchema#string"/>
  </owl:DatatypeProperty>
  <owl:DatatypeProperty rdf:about="http://example.org/onto/prop/google_cloudfunctions_function_delete">
    <rdfs:label>delete</rdfs:label>
    <rdfs:domain rdf:resource="http://example.org/onto/class/google_cloudfunctions_function"/>
    <rdfs:range rdf:resource="http://www.w3.org/2001/XMLSchema#string"/>
  </owl:DatatypeProperty>
  <owl:DatatypeProperty rdf:about="http://example.org/onto/prop/google_cloudfunctions_function_read">
    <rdfs:label>read</rdfs:label>
    <rdfs:domain rdf:resource="http://example.org/onto/class/google_cloudfunctions_function"/>
    <rdfs:range rdf:resource="http://www.w3.org/2001/XMLSchema#string"/>
  </owl:DatatypeProperty>
  <owl:DatatypeProperty rdf:about="http://example.org/onto/prop/google_cloudfunctions_function_update">
    <rdfs:label>update</rdfs:label>
    <rdfs:domain rdf:resource="http://example.org/onto/class/google_cloudfunctions_function"/>
    <rdfs:range rdf:resource="http://www.w3.org/2001/XMLSchema#string"/>
  </owl:DatatypeProperty>
</rdf:RDF>
