<?xml version="1.0" encoding="UTF-8"?>
<rdf:RDF
  xmlns:rdf="http://www.w3.org/1999/02/22-rdf-syntax-ns#"
  xmlns:rdfs="http://www.w3.org/2000/01/rdf-schema#"
  xmlns:owl="http://www.w3.org/2002/07/owl#"
  xmlns:xsd="http://www.w3.org/2001/XMLSchema#"
  xml:base="http://example.org/onto/">
  <owl:Class rdf:about="http://example.org/onto/class/yandex_mdb_greenplum_resource_group">
    <rdfs:label>yandex_mdb_greenplum_resource_group</rdfs:label>
    <rdfs:comment>Manages a Greenplum resource group within the Yandex Cloud. For more information, see [the official documentation](https://yandex.cloud/docs/managed-greenplum/).</rdfs:comment>
  </owl:Class>
  <owl:DatatypeProperty rdf:about="http://example.org/onto/prop/yandex_mdb_greenplum_resource_group_cluster_id">
    <rdfs:label>cluster_id</rdfs:label>
    <rdfs:comment>The ID of the cluster to which resource group belongs to.</rdfs:comment>
    <rdfs:domain rdf:resource="http://example.org/onto/class/yandex_mdb_greenplum_resource_group"/>
    <rdfs:range rdf:resource="http://www.w3.org/2001/XMLSchema#string"/>
  </owl:DatatypeProperty>
  <owl:DatatypeProperty rdf:about="http://example.org/onto/prop/yandex_mdb_greenplum_resource_group_concurrency">
    <rdfs:label>concurrency</rdfs:label>
    <rdfs:comment>The maximum number of concurrent transactions, including active and idle transactions, that are permitted in the resource group.</rdfs:comment>
    <rdfs:domain rdf:resource="http://example.org/onto/class/yandex_mdb_greenplum_resource_group"/>
    <rdfs:range rdf:resource="http://www.w3.org/2001/XMLSchema#string"/>
  </owl:DatatypeProperty>
  <owl:DatatypeProperty rdf:about="http://example.org/onto/prop/yandex_mdb_greenplum_resource_group_cpu_rate_limit">
    <rdfs:label>cpu_rate_limit</rdfs:label>
    <rdfs:comment>The percentage of CPU resources available to this resource group.</rdfs:comment>
    <rdfs:domain rdf:resource="http://example.org/onto/class/yandex_mdb_greenplum_resource_group"/>
    <rdfs:range rdf:resource="http://www.w3.org/2001/XMLSchema#string"/>
  </owl:DatatypeProperty>
  <owl:DatatypeProperty rdf:about="http://example.org/onto/prop/yandex_mdb_greenplum_resource_group_id">
    <rdfs:label>id</rdfs:label>
    <rdfs:comment>The resource identifier.</rdfs:comment>
    <rdfs:domain rdf:resource="http://example.org/onto/class/yandex_mdb_greenplum_resource_group"/>
    <rdfs:range rdf:resource="http://www.w3.org/2001/XMLSchema#string"/>
  </owl:DatatypeProperty>
  <owl:DatatypeProperty rdf:about="http://example.org/onto/prop/yandex_mdb_greenplum_resource_group_is_user_defined">
    <rdfs:label>is_user_defined</rdfs:label>
    <rdfs:comment>If false, the resource group is immutable and controlled by yandex</rdfs:comment>
    <rdfs:domain rdf:resource="http://example.org/onto/class/yandex_mdb_greenplum_resource_group"/>
    <rdfs:range rdf:resource="http://www.w3.org/2001/XMLSchema#string"/>
  </owl:DatatypeProperty>
  <owl:DatatypeProperty rdf:about="http://example.org/onto/prop/yandex_mdb_greenplum_resource_group_memory_limit">
    <rdfs:label>memory_limit</rdfs:label>
    <rdfs:comment>The percentage of reserved memory resources available to this resource group.</rdfs:comment>
    <rdfs:domain rdf:resource="http://example.org/onto/class/yandex_mdb_greenplum_resource_group"/>
    <rdfs:range rdf:resource="http://www.w3.org/2001/XMLSchema#string"/>
  </owl:DatatypeProperty>
  <owl:DatatypeProperty rdf:about="http://example.org/onto/prop/yandex_mdb_greenplum_resource_group_memory_shared_quota">
    <rdfs:label>memory_shared_quota</rdfs:label>
    <rdfs:comment>The percentage of reserved memory to share across transactions submitted in this resource group.</rdfs:comment>
    <rdfs:domain rdf:resource="http://example.org/onto/class/yandex_mdb_greenplum_resource_group"/>
    <rdfs:range rdf:resource="http://www.w3.org/2001/XMLSchema#string"/>
  </owl:DatatypeProperty>
  <owl:DatatypeProperty rdf:about="http://example.org/onto/prop/yandex_mdb_greenplum_resource_group_memory_spill_ratio">
    <rdfs:label>memory_spill_ratio</rdfs:label>
    <rdfs:comment>The memory usage threshold for memory-intensive transactions. When a transaction reaches this threshold, it spills to disk.</rdfs:comment>
    <rdfs:domain rdf:resource="http://example.org/onto/class/yandex_mdb_greenplum_resource_group"/>
    <rdfs:range rdf:resource="http://www.w3.org/2001/XMLSchema#string"/>
  </owl:DatatypeProperty>
  <owl:DatatypeProperty rdf:about="http://example.org/onto/prop/yandex_mdb_greenplum_resource_group_name">
    <rdfs:label>name</rdfs:label>
    <rdfs:comment>The name of the resource group.</rdfs:comment>
    <rdfs:domain rdf:resource="http://example.org/onto/class/yandex_mdb_greenplum_resource_group"/>
    <rdfs:range rdf:resource="http://www.w3.org/2001/XMLSchema#string"/>
  </owl:DatatypeProperty>
  <owl:DatatypeProperty rdf:about="http://example.org/onto/prop/yandex_mdb_greenplum_resource_group_timeouts">
    <rdfs:label>timeouts</rdfs:label>
    <rdfs:domain rdf:resource="http://example.org/onto/class/yandex_mdb_greenplum_resource_group"/>
    <rdfs:range rdf:resource="http://www.w3.org/2001/XMLSchema#string"/>
  </owl:DatatypeProperty>
</rdf:RDF>
