<?xml version="1.0" encoding="UTF-8"?>
<rdf:RDF
  xmlns:rdf="http://www.w3.org/1999/02/22-rdf-syntax-ns#"
  xmlns:rdfs="http://www.w3.org/2000/01/rdf-schema#"
  xmlns:owl="http://www.w3.org/2002/07/owl#"
  xmlns:xsd="http://www.w3.org/2001/XMLSchema#"
  xml:base="http://example.org/onto/">
  <owl:Class rdf:about="http://example.org/onto/class/yandex_storage_bucket_grant">
    <rdfs:label>yandex_storage_bucket_grant</rdfs:label>
    <rdfs:comment>Allows management of grants on an existing [Yandex Cloud Storage Bucket](https://yandex.cloud/docs/storage/concepts/bucket).

~> By default, for authentication, you need to use [IAM token](https://yandex.cloud/docs/iam/concepts/authorization/iam-token) with the necessary permissions.

~> Alternatively, you can provide [static access keys](https://yandex.cloud/docs/iam/concepts/authorization/access-key) (Access and Secret). To generate these keys, you will need a Service Account with the appropriate permissions.

This resource should be used for managing [Primitive roles](https://yandex.cloud/docs/storage/security/#primitive-roles) only.

Declaring multiple yandex_storage_bucket_grant resources to the same bucket will cause a perpetual difference in configuration.</rdfs:comment>
  </owl:Class>
  <owl:DatatypeProperty rdf:about="http://example.org/onto/prop/yandex_storage_bucket_grant_access_key">
    <rdfs:label>access_key</rdfs:label>
    <rdfs:comment>The access key to use when applying changes. This value can also be provided as `storage_access_key` specified in provider config (explicitly or within `shared_credentials_file`) is used.</rdfs:comment>
    <rdfs:domain rdf:resource="http://example.org/onto/class/yandex_storage_bucket_grant"/>
    <rdfs:range rdf:resource="http://www.w3.org/2001/XMLSchema#string"/>
  </owl:DatatypeProperty>
  <owl:DatatypeProperty rdf:about="http://example.org/onto/prop/yandex_storage_bucket_grant_acl">
    <rdfs:label>acl</rdfs:label>
    <rdfs:comment>The [predefined ACL](https://yandex.cloud/docs/storage/concepts/acl#predefined_acls) to apply. Defaults to `private`. Conflicts with `grant`.

~> To change ACL after creation, service account with `storage.admin` role should be used, though this role is not necessary to create a bucket with any ACL.</rdfs:comment>
    <rdfs:domain rdf:resource="http://example.org/onto/class/yandex_storage_bucket_grant"/>
    <rdfs:range rdf:resource="http://www.w3.org/2001/XMLSchema#string"/>
  </owl:DatatypeProperty>
  <owl:DatatypeProperty rdf:about="http://example.org/onto/prop/yandex_storage_bucket_grant_bucket">
    <rdfs:label>bucket</rdfs:label>
    <rdfs:comment>The name of the bucket.</rdfs:comment>
    <rdfs:domain rdf:resource="http://example.org/onto/class/yandex_storage_bucket_grant"/>
    <rdfs:range rdf:resource="http://www.w3.org/2001/XMLSchema#string"/>
  </owl:DatatypeProperty>
  <owl:DatatypeProperty rdf:about="http://example.org/onto/prop/yandex_storage_bucket_grant_secret_key">
    <rdfs:label>secret_key</rdfs:label>
    <rdfs:comment>The secret key to use when applying changes. This value can also be provided as `storage_secret_key` specified in provider config (explicitly or within `shared_credentials_file`) is used.</rdfs:comment>
    <rdfs:domain rdf:resource="http://example.org/onto/class/yandex_storage_bucket_grant"/>
    <rdfs:range rdf:resource="http://www.w3.org/2001/XMLSchema#string"/>
  </owl:DatatypeProperty>
  <owl:DatatypeProperty rdf:about="http://example.org/onto/prop/yandex_storage_bucket_grant_id">
    <rdfs:label>id</rdfs:label>
    <rdfs:comment>Canonical user id to grant for. Used only when type is `CanonicalUser`.</rdfs:comment>
    <rdfs:domain rdf:resource="http://example.org/onto/class/yandex_storage_bucket_grant"/>
    <rdfs:range rdf:resource="http://www.w3.org/2001/XMLSchema#string"/>
  </owl:DatatypeProperty>
  <owl:DatatypeProperty rdf:about="http://example.org/onto/prop/yandex_storage_bucket_grant_permissions">
    <rdfs:label>permissions</rdfs:label>
    <rdfs:comment>List of permissions to apply for grantee. Valid values are `READ`, `WRITE`, `FULL_CONTROL`.</rdfs:comment>
    <rdfs:domain rdf:resource="http://example.org/onto/class/yandex_storage_bucket_grant"/>
    <rdfs:range rdf:resource="http://www.w3.org/2001/XMLSchema#string"/>
  </owl:DatatypeProperty>
  <owl:DatatypeProperty rdf:about="http://example.org/onto/prop/yandex_storage_bucket_grant_type">
    <rdfs:label>type</rdfs:label>
    <rdfs:comment>Type of grantee to apply for. Valid values are `CanonicalUser` and `Group`.</rdfs:comment>
    <rdfs:domain rdf:resource="http://example.org/onto/class/yandex_storage_bucket_grant"/>
    <rdfs:range rdf:resource="http://www.w3.org/2001/XMLSchema#string"/>
  </owl:DatatypeProperty>
  <owl:DatatypeProperty rdf:about="http://example.org/onto/prop/yandex_storage_bucket_grant_uri">
    <rdfs:label>uri</rdfs:label>
    <rdfs:comment>URI address to grant for. Used only when type is Group.</rdfs:comment>
    <rdfs:domain rdf:resource="http://example.org/onto/class/yandex_storage_bucket_grant"/>
    <rdfs:range rdf:resource="http://www.w3.org/2001/XMLSchema#string"/>
  </owl:DatatypeProperty>
</rdf:RDF>
