<?xml version="1.0" encoding="UTF-8"?>
<rdf:RDF
  xmlns:rdf="http://www.w3.org/1999/02/22-rdf-syntax-ns#"
  xmlns:rdfs="http://www.w3.org/2000/01/rdf-schema#"
  xmlns:owl="http://www.w3.org/2002/07/owl#"
  xmlns:xsd="http://www.w3.org/2001/XMLSchema#"
  xml:base="http://example.org/onto/">
  <owl:Class rdf:about="http://example.org/onto/class/yandex_lb_target_group">
    <rdfs:label>yandex_lb_target_group</rdfs:label>
    <rdfs:comment>A TargetGroup resource. For more information, see [Target groups and resources](/docs/network-load-balancer/concepts/target-resources).</rdfs:comment>
  </owl:Class>
  <owl:DatatypeProperty rdf:about="http://example.org/onto/prop/yandex_lb_target_group_created_at">
    <rdfs:label>created_at</rdfs:label>
    <rdfs:comment>Output only. Creation timestamp in [RFC3339](https://www.ietf.org/rfc/rfc3339.txt) text format.</rdfs:comment>
    <rdfs:domain rdf:resource="http://example.org/onto/class/yandex_lb_target_group"/>
    <rdfs:range rdf:resource="http://www.w3.org/2001/XMLSchema#string"/>
  </owl:DatatypeProperty>
  <owl:DatatypeProperty rdf:about="http://example.org/onto/prop/yandex_lb_target_group_description">
    <rdfs:label>description</rdfs:label>
    <rdfs:comment>Description of the target group. 0-256 characters long.</rdfs:comment>
    <rdfs:domain rdf:resource="http://example.org/onto/class/yandex_lb_target_group"/>
    <rdfs:range rdf:resource="http://www.w3.org/2001/XMLSchema#string"/>
  </owl:DatatypeProperty>
  <owl:DatatypeProperty rdf:about="http://example.org/onto/prop/yandex_lb_target_group_folder_id">
    <rdfs:label>folder_id</rdfs:label>
    <rdfs:comment>ID of the folder that the target group belongs to.</rdfs:comment>
    <rdfs:domain rdf:resource="http://example.org/onto/class/yandex_lb_target_group"/>
    <rdfs:range rdf:resource="http://www.w3.org/2001/XMLSchema#string"/>
  </owl:DatatypeProperty>
  <owl:DatatypeProperty rdf:about="http://example.org/onto/prop/yandex_lb_target_group_id">
    <rdfs:label>id</rdfs:label>
    <rdfs:comment>ID of the TargetGroup resource to return.
 To get the target group ID, use a [TargetGroupService.List] request.</rdfs:comment>
    <rdfs:domain rdf:resource="http://example.org/onto/class/yandex_lb_target_group"/>
    <rdfs:range rdf:resource="http://www.w3.org/2001/XMLSchema#string"/>
  </owl:DatatypeProperty>
  <owl:DatatypeProperty rdf:about="http://example.org/onto/prop/yandex_lb_target_group_labels">
    <rdfs:label>labels</rdfs:label>
    <rdfs:comment>Resource labels as `` key:value `` pairs. Maximum of 64 per resource.</rdfs:comment>
    <rdfs:domain rdf:resource="http://example.org/onto/class/yandex_lb_target_group"/>
    <rdfs:range rdf:resource="http://www.w3.org/2001/XMLSchema#string"/>
  </owl:DatatypeProperty>
  <owl:DatatypeProperty rdf:about="http://example.org/onto/prop/yandex_lb_target_group_name">
    <rdfs:label>name</rdfs:label>
    <rdfs:comment>Name of the target group.
 The name is unique within the folder. 3-63 characters long.</rdfs:comment>
    <rdfs:domain rdf:resource="http://example.org/onto/class/yandex_lb_target_group"/>
    <rdfs:range rdf:resource="http://www.w3.org/2001/XMLSchema#string"/>
  </owl:DatatypeProperty>
  <owl:DatatypeProperty rdf:about="http://example.org/onto/prop/yandex_lb_target_group_region_id">
    <rdfs:label>region_id</rdfs:label>
    <rdfs:comment>ID of the region where the target group resides.</rdfs:comment>
    <rdfs:domain rdf:resource="http://example.org/onto/class/yandex_lb_target_group"/>
    <rdfs:range rdf:resource="http://www.w3.org/2001/XMLSchema#string"/>
  </owl:DatatypeProperty>
  <owl:DatatypeProperty rdf:about="http://example.org/onto/prop/yandex_lb_target_group_target_group_id">
    <rdfs:label>target_group_id</rdfs:label>
    <rdfs:comment>ID of the TargetGroup resource to return.
 To get the target group ID, use a [TargetGroupService.List] request.</rdfs:comment>
    <rdfs:domain rdf:resource="http://example.org/onto/class/yandex_lb_target_group"/>
    <rdfs:range rdf:resource="http://www.w3.org/2001/XMLSchema#string"/>
  </owl:DatatypeProperty>
  <owl:DatatypeProperty rdf:about="http://example.org/onto/prop/yandex_lb_target_group_address">
    <rdfs:label>address</rdfs:label>
    <rdfs:comment>IP address of the target.</rdfs:comment>
    <rdfs:domain rdf:resource="http://example.org/onto/class/yandex_lb_target_group"/>
    <rdfs:range rdf:resource="http://www.w3.org/2001/XMLSchema#string"/>
  </owl:DatatypeProperty>
  <owl:DatatypeProperty rdf:about="http://example.org/onto/prop/yandex_lb_target_group_subnet_id">
    <rdfs:label>subnet_id</rdfs:label>
    <rdfs:comment>ID of the subnet that targets are connected to.
 All targets in the target group must be connected to the same subnet within a single availability zone.</rdfs:comment>
    <rdfs:domain rdf:resource="http://example.org/onto/class/yandex_lb_target_group"/>
    <rdfs:range rdf:resource="http://www.w3.org/2001/XMLSchema#string"/>
  </owl:DatatypeProperty>
  <owl:DatatypeProperty rdf:about="http://example.org/onto/prop/yandex_lb_target_group_create">
    <rdfs:label>create</rdfs:label>
    <rdfs:comment>A string that can be [parsed as a duration](https://pkg.go.dev/time#ParseDuration) consisting of numbers and unit suffixes, such as "30s" or "2h45m". Valid time units are "s" (seconds), "m" (minutes), "h" (hours).</rdfs:comment>
    <rdfs:domain rdf:resource="http://example.org/onto/class/yandex_lb_target_group"/>
    <rdfs:range rdf:resource="http://www.w3.org/2001/XMLSchema#string"/>
  </owl:DatatypeProperty>
  <owl:DatatypeProperty rdf:about="http://example.org/onto/prop/yandex_lb_target_group_delete">
    <rdfs:label>delete</rdfs:label>
    <rdfs:comment>A string that can be [parsed as a duration](https://pkg.go.dev/time#ParseDuration) consisting of numbers and unit suffixes, such as "30s" or "2h45m". Valid time units are "s" (seconds), "m" (minutes), "h" (hours). Setting a timeout for a Delete operation is only applicable if changes are saved into state before the destroy operation occurs.</rdfs:comment>
    <rdfs:domain rdf:resource="http://example.org/onto/class/yandex_lb_target_group"/>
    <rdfs:range rdf:resource="http://www.w3.org/2001/XMLSchema#string"/>
  </owl:DatatypeProperty>
  <owl:DatatypeProperty rdf:about="http://example.org/onto/prop/yandex_lb_target_group_read">
    <rdfs:label>read</rdfs:label>
    <rdfs:comment>A string that can be [parsed as a duration](https://pkg.go.dev/time#ParseDuration) consisting of numbers and unit suffixes, such as "30s" or "2h45m". Valid time units are "s" (seconds), "m" (minutes), "h" (hours). Read operations occur during any refresh or planning operation when refresh is enabled.</rdfs:comment>
    <rdfs:domain rdf:resource="http://example.org/onto/class/yandex_lb_target_group"/>
    <rdfs:range rdf:resource="http://www.w3.org/2001/XMLSchema#string"/>
  </owl:DatatypeProperty>
  <owl:DatatypeProperty rdf:about="http://example.org/onto/prop/yandex_lb_target_group_update">
    <rdfs:label>update</rdfs:label>
    <rdfs:comment>A string that can be [parsed as a duration](https://pkg.go.dev/time#ParseDuration) consisting of numbers and unit suffixes, such as "30s" or "2h45m". Valid time units are "s" (seconds), "m" (minutes), "h" (hours).</rdfs:comment>
    <rdfs:domain rdf:resource="http://example.org/onto/class/yandex_lb_target_group"/>
    <rdfs:range rdf:resource="http://www.w3.org/2001/XMLSchema#string"/>
  </owl:DatatypeProperty>
</rdf:RDF>
