<?xml version="1.0" encoding="UTF-8"?>
<rdf:RDF
  xmlns:rdf="http://www.w3.org/1999/02/22-rdf-syntax-ns#"
  xmlns:rdfs="http://www.w3.org/2000/01/rdf-schema#"
  xmlns:owl="http://www.w3.org/2002/07/owl#"
  xmlns:xsd="http://www.w3.org/2001/XMLSchema#"
  xml:base="http://example.org/onto/">
  <owl:Class rdf:about="http://example.org/onto/class/yandex_mdb_mongodb_cluster">
    <rdfs:label>yandex_mdb_mongodb_cluster</rdfs:label>
    <rdfs:comment>Manages a MongoDB cluster within the Yandex Cloud. For more information, see [the official documentation](https://yandex.cloud/docs/managed-mongodb/concepts).</rdfs:comment>
  </owl:Class>
  <owl:DatatypeProperty rdf:about="http://example.org/onto/prop/yandex_mdb_mongodb_cluster_cluster_id">
    <rdfs:label>cluster_id</rdfs:label>
    <rdfs:comment>The ID of the cluster.</rdfs:comment>
    <rdfs:domain rdf:resource="http://example.org/onto/class/yandex_mdb_mongodb_cluster"/>
    <rdfs:range rdf:resource="http://www.w3.org/2001/XMLSchema#string"/>
  </owl:DatatypeProperty>
  <owl:DatatypeProperty rdf:about="http://example.org/onto/prop/yandex_mdb_mongodb_cluster_created_at">
    <rdfs:label>created_at</rdfs:label>
    <rdfs:comment>The creation timestamp of the resource.</rdfs:comment>
    <rdfs:domain rdf:resource="http://example.org/onto/class/yandex_mdb_mongodb_cluster"/>
    <rdfs:range rdf:resource="http://www.w3.org/2001/XMLSchema#string"/>
  </owl:DatatypeProperty>
  <owl:DatatypeProperty rdf:about="http://example.org/onto/prop/yandex_mdb_mongodb_cluster_deletion_protection">
    <rdfs:label>deletion_protection</rdfs:label>
    <rdfs:comment>The `true` value means that resource is protected from accidental deletion.</rdfs:comment>
    <rdfs:domain rdf:resource="http://example.org/onto/class/yandex_mdb_mongodb_cluster"/>
    <rdfs:range rdf:resource="http://www.w3.org/2001/XMLSchema#string"/>
  </owl:DatatypeProperty>
  <owl:DatatypeProperty rdf:about="http://example.org/onto/prop/yandex_mdb_mongodb_cluster_description">
    <rdfs:label>description</rdfs:label>
    <rdfs:comment>The resource description.</rdfs:comment>
    <rdfs:domain rdf:resource="http://example.org/onto/class/yandex_mdb_mongodb_cluster"/>
    <rdfs:range rdf:resource="http://www.w3.org/2001/XMLSchema#string"/>
  </owl:DatatypeProperty>
  <owl:DatatypeProperty rdf:about="http://example.org/onto/prop/yandex_mdb_mongodb_cluster_disk_encryption_key_id">
    <rdfs:label>disk_encryption_key_id</rdfs:label>
    <rdfs:comment>ID of the KMS key for cluster disk encryption.</rdfs:comment>
    <rdfs:domain rdf:resource="http://example.org/onto/class/yandex_mdb_mongodb_cluster"/>
    <rdfs:range rdf:resource="http://www.w3.org/2001/XMLSchema#string"/>
  </owl:DatatypeProperty>
  <owl:DatatypeProperty rdf:about="http://example.org/onto/prop/yandex_mdb_mongodb_cluster_environment">
    <rdfs:label>environment</rdfs:label>
    <rdfs:comment>Deployment environment of the MongoDB cluster. Can be either `PRESTABLE` or `PRODUCTION`.</rdfs:comment>
    <rdfs:domain rdf:resource="http://example.org/onto/class/yandex_mdb_mongodb_cluster"/>
    <rdfs:range rdf:resource="http://www.w3.org/2001/XMLSchema#string"/>
  </owl:DatatypeProperty>
  <owl:DatatypeProperty rdf:about="http://example.org/onto/prop/yandex_mdb_mongodb_cluster_folder_id">
    <rdfs:label>folder_id</rdfs:label>
    <rdfs:comment>The folder identifier that resource belongs to. If it is not provided, the default provider `folder-id` is used.</rdfs:comment>
    <rdfs:domain rdf:resource="http://example.org/onto/class/yandex_mdb_mongodb_cluster"/>
    <rdfs:range rdf:resource="http://www.w3.org/2001/XMLSchema#string"/>
  </owl:DatatypeProperty>
  <owl:DatatypeProperty rdf:about="http://example.org/onto/prop/yandex_mdb_mongodb_cluster_health">
    <rdfs:label>health</rdfs:label>
    <rdfs:comment>Aggregated health of the cluster. Can be either `ALIVE`, `DEGRADED`, `DEAD` or `HEALTH_UNKNOWN`. For more information see `health` field of JSON representation in [the official documentation](https://yandex.cloud/docs/managed-mongodb/api-ref/Cluster/).</rdfs:comment>
    <rdfs:domain rdf:resource="http://example.org/onto/class/yandex_mdb_mongodb_cluster"/>
    <rdfs:range rdf:resource="http://www.w3.org/2001/XMLSchema#string"/>
  </owl:DatatypeProperty>
  <owl:DatatypeProperty rdf:about="http://example.org/onto/prop/yandex_mdb_mongodb_cluster_id">
    <rdfs:label>id</rdfs:label>
    <rdfs:domain rdf:resource="http://example.org/onto/class/yandex_mdb_mongodb_cluster"/>
    <rdfs:range rdf:resource="http://www.w3.org/2001/XMLSchema#string"/>
  </owl:DatatypeProperty>
  <owl:DatatypeProperty rdf:about="http://example.org/onto/prop/yandex_mdb_mongodb_cluster_labels">
    <rdfs:label>labels</rdfs:label>
    <rdfs:comment>A set of key/value label pairs which assigned to resource.</rdfs:comment>
    <rdfs:domain rdf:resource="http://example.org/onto/class/yandex_mdb_mongodb_cluster"/>
    <rdfs:range rdf:resource="http://www.w3.org/2001/XMLSchema#string"/>
  </owl:DatatypeProperty>
  <owl:DatatypeProperty rdf:about="http://example.org/onto/prop/yandex_mdb_mongodb_cluster_name">
    <rdfs:label>name</rdfs:label>
    <rdfs:comment>The resource name.</rdfs:comment>
    <rdfs:domain rdf:resource="http://example.org/onto/class/yandex_mdb_mongodb_cluster"/>
    <rdfs:range rdf:resource="http://www.w3.org/2001/XMLSchema#string"/>
  </owl:DatatypeProperty>
  <owl:DatatypeProperty rdf:about="http://example.org/onto/prop/yandex_mdb_mongodb_cluster_network_id">
    <rdfs:label>network_id</rdfs:label>
    <rdfs:comment>The `VPC Network ID` of subnets which resource attached to.</rdfs:comment>
    <rdfs:domain rdf:resource="http://example.org/onto/class/yandex_mdb_mongodb_cluster"/>
    <rdfs:range rdf:resource="http://www.w3.org/2001/XMLSchema#string"/>
  </owl:DatatypeProperty>
  <owl:DatatypeProperty rdf:about="http://example.org/onto/prop/yandex_mdb_mongodb_cluster_security_group_ids">
    <rdfs:label>security_group_ids</rdfs:label>
    <rdfs:comment>The list of security groups applied to resource or their components.</rdfs:comment>
    <rdfs:domain rdf:resource="http://example.org/onto/class/yandex_mdb_mongodb_cluster"/>
    <rdfs:range rdf:resource="http://www.w3.org/2001/XMLSchema#string"/>
  </owl:DatatypeProperty>
  <owl:DatatypeProperty rdf:about="http://example.org/onto/prop/yandex_mdb_mongodb_cluster_sharded">
    <rdfs:label>sharded</rdfs:label>
    <rdfs:comment>MongoDB Cluster mode enabled/disabled.</rdfs:comment>
    <rdfs:domain rdf:resource="http://example.org/onto/class/yandex_mdb_mongodb_cluster"/>
    <rdfs:range rdf:resource="http://www.w3.org/2001/XMLSchema#string"/>
  </owl:DatatypeProperty>
  <owl:DatatypeProperty rdf:about="http://example.org/onto/prop/yandex_mdb_mongodb_cluster_status">
    <rdfs:label>status</rdfs:label>
    <rdfs:comment>Status of the cluster. Can be either `CREATING`, `STARTING`, `RUNNING`, `UPDATING`, `STOPPING`, `STOPPED`, `ERROR` or `STATUS_UNKNOWN`. For more information see `status` field of JSON representation in [the official documentation](https://yandex.cloud/docs/managed-mongodb/api-ref/Cluster/).</rdfs:comment>
    <rdfs:domain rdf:resource="http://example.org/onto/class/yandex_mdb_mongodb_cluster"/>
    <rdfs:range rdf:resource="http://www.w3.org/2001/XMLSchema#string"/>
  </owl:DatatypeProperty>
  <owl:DatatypeProperty rdf:about="http://example.org/onto/prop/yandex_mdb_mongodb_cluster_backup_retain_period_days">
    <rdfs:label>backup_retain_period_days</rdfs:label>
    <rdfs:comment>Retain period of automatically created backup in days.</rdfs:comment>
    <rdfs:domain rdf:resource="http://example.org/onto/class/yandex_mdb_mongodb_cluster"/>
    <rdfs:range rdf:resource="http://www.w3.org/2001/XMLSchema#string"/>
  </owl:DatatypeProperty>
  <owl:DatatypeProperty rdf:about="http://example.org/onto/prop/yandex_mdb_mongodb_cluster_feature_compatibility_version">
    <rdfs:label>feature_compatibility_version</rdfs:label>
    <rdfs:comment>Feature compatibility version of MongoDB. If not provided version is taken. Can be either `6.0`, `5.0`, `4.4` and `4.2`.</rdfs:comment>
    <rdfs:domain rdf:resource="http://example.org/onto/class/yandex_mdb_mongodb_cluster"/>
    <rdfs:range rdf:resource="http://www.w3.org/2001/XMLSchema#string"/>
  </owl:DatatypeProperty>
  <owl:DatatypeProperty rdf:about="http://example.org/onto/prop/yandex_mdb_mongodb_cluster_version">
    <rdfs:label>version</rdfs:label>
    <rdfs:comment>Version of the MongoDB server software. Can be either `4.2`, `4.4`, `4.4-enterprise`, `5.0`, `5.0-enterprise`, `6.0` and `6.0-enterprise`.</rdfs:comment>
    <rdfs:domain rdf:resource="http://example.org/onto/class/yandex_mdb_mongodb_cluster"/>
    <rdfs:range rdf:resource="http://www.w3.org/2001/XMLSchema#string"/>
  </owl:DatatypeProperty>
  <owl:DatatypeProperty rdf:about="http://example.org/onto/prop/yandex_mdb_mongodb_cluster_data_lens">
    <rdfs:label>data_lens</rdfs:label>
    <rdfs:comment>Allow access for [Yandex DataLens](https://yandex.cloud/services/datalens).</rdfs:comment>
    <rdfs:domain rdf:resource="http://example.org/onto/class/yandex_mdb_mongodb_cluster"/>
    <rdfs:range rdf:resource="http://www.w3.org/2001/XMLSchema#string"/>
  </owl:DatatypeProperty>
  <owl:DatatypeProperty rdf:about="http://example.org/onto/prop/yandex_mdb_mongodb_cluster_data_transfer">
    <rdfs:label>data_transfer</rdfs:label>
    <rdfs:comment>Allow access for [DataTransfer](https://yandex.cloud/services/data-transfer).</rdfs:comment>
    <rdfs:domain rdf:resource="http://example.org/onto/class/yandex_mdb_mongodb_cluster"/>
    <rdfs:range rdf:resource="http://www.w3.org/2001/XMLSchema#string"/>
  </owl:DatatypeProperty>
  <owl:DatatypeProperty rdf:about="http://example.org/onto/prop/yandex_mdb_mongodb_cluster_web_sql">
    <rdfs:label>web_sql</rdfs:label>
    <rdfs:comment>Allow access for [WebSQL](https://yandex.cloud/ru/docs/websql/).</rdfs:comment>
    <rdfs:domain rdf:resource="http://example.org/onto/class/yandex_mdb_mongodb_cluster"/>
    <rdfs:range rdf:resource="http://www.w3.org/2001/XMLSchema#string"/>
  </owl:DatatypeProperty>
  <owl:DatatypeProperty rdf:about="http://example.org/onto/prop/yandex_mdb_mongodb_cluster_hours">
    <rdfs:label>hours</rdfs:label>
    <rdfs:comment>The hour at which backup will be started.</rdfs:comment>
    <rdfs:domain rdf:resource="http://example.org/onto/class/yandex_mdb_mongodb_cluster"/>
    <rdfs:range rdf:resource="http://www.w3.org/2001/XMLSchema#string"/>
  </owl:DatatypeProperty>
  <owl:DatatypeProperty rdf:about="http://example.org/onto/prop/yandex_mdb_mongodb_cluster_minutes">
    <rdfs:label>minutes</rdfs:label>
    <rdfs:comment>The minute at which backup will be started.</rdfs:comment>
    <rdfs:domain rdf:resource="http://example.org/onto/class/yandex_mdb_mongodb_cluster"/>
    <rdfs:range rdf:resource="http://www.w3.org/2001/XMLSchema#string"/>
  </owl:DatatypeProperty>
  <owl:DatatypeProperty rdf:about="http://example.org/onto/prop/yandex_mdb_mongodb_cluster_max_incoming_connections">
    <rdfs:label>max_incoming_connections</rdfs:label>
    <rdfs:comment>The maximum number of simultaneous connections that host will accept. For more information, see the [net.maxIncomingConnections](https://www.mongodb.com/docs/manual/reference/configuration-options/#mongodb-setting-net.maxIncomingConnections) description in the official documentation.</rdfs:comment>
    <rdfs:domain rdf:resource="http://example.org/onto/class/yandex_mdb_mongodb_cluster"/>
    <rdfs:range rdf:resource="http://www.w3.org/2001/XMLSchema#string"/>
  </owl:DatatypeProperty>
  <owl:DatatypeProperty rdf:about="http://example.org/onto/prop/yandex_mdb_mongodb_cluster_mode">
    <rdfs:label>mode</rdfs:label>
    <rdfs:comment>Specifies which operations should be profiled. The following profiler levels are available: off, slow_op, all. For more information, see the [operationProfiling.mode](https://www.mongodb.com/docs/manual/reference/configuration-options/#mongodb-setting-operationProfiling.mode) description in the official documentation.</rdfs:comment>
    <rdfs:domain rdf:resource="http://example.org/onto/class/yandex_mdb_mongodb_cluster"/>
    <rdfs:range rdf:resource="http://www.w3.org/2001/XMLSchema#string"/>
  </owl:DatatypeProperty>
  <owl:DatatypeProperty rdf:about="http://example.org/onto/prop/yandex_mdb_mongodb_cluster_slow_op_threshold">
    <rdfs:label>slow_op_threshold</rdfs:label>
    <rdfs:comment>The slow operation time threshold, in milliseconds. Operations that run for longer than this threshold are considered slow. For more information, see the [operationProfiling.slowOpThresholdMs](https://www.mongodb.com/docs/manual/reference/configuration-options/#mongodb-setting-operationProfiling.slowOpThresholdMs) description in the official documentation.</rdfs:comment>
    <rdfs:domain rdf:resource="http://example.org/onto/class/yandex_mdb_mongodb_cluster"/>
    <rdfs:range rdf:resource="http://www.w3.org/2001/XMLSchema#string"/>
  </owl:DatatypeProperty>
  <owl:DatatypeProperty rdf:about="http://example.org/onto/prop/yandex_mdb_mongodb_cluster_cache_size_gb">
    <rdfs:label>cache_size_gb</rdfs:label>
    <rdfs:comment>Defines the maximum size of the internal cache that WiredTiger will use for all data. For more information, see the [storage.wiredTiger.engineConfig.cacheSizeGB](https://www.mongodb.com/docs/manual/reference/configuration-options/#mongodb-setting-storage.wiredTiger.engineConfig.cacheSizeGB) description in the official documentation.</rdfs:comment>
    <rdfs:domain rdf:resource="http://example.org/onto/class/yandex_mdb_mongodb_cluster"/>
    <rdfs:range rdf:resource="http://www.w3.org/2001/XMLSchema#string"/>
  </owl:DatatypeProperty>
  <owl:DatatypeProperty rdf:about="http://example.org/onto/prop/yandex_mdb_mongodb_cluster_filter">
    <rdfs:label>filter</rdfs:label>
    <rdfs:comment>Configuration of the audit log filter in JSON format. For more information see [auditLog.filter](https://www.mongodb.com/docs/manual/reference/configuration-options/#mongodb-setting-auditLog.filter) description in the official documentation. Available only in enterprise edition.</rdfs:comment>
    <rdfs:domain rdf:resource="http://example.org/onto/class/yandex_mdb_mongodb_cluster"/>
    <rdfs:range rdf:resource="http://www.w3.org/2001/XMLSchema#string"/>
  </owl:DatatypeProperty>
  <owl:DatatypeProperty rdf:about="http://example.org/onto/prop/yandex_mdb_mongodb_cluster_runtime_configuration">
    <rdfs:label>runtime_configuration</rdfs:label>
    <rdfs:comment>Specifies if a node allows runtime configuration of audit filters and the auditAuthorizationSuccess variable. For more information see [auditLog.runtimeConfiguration](https://www.mongodb.com/docs/manual/reference/configuration-options/#mongodb-setting-auditLog.runtimeConfiguration) description in the official documentation. Available only in enterprise edition.</rdfs:comment>
    <rdfs:domain rdf:resource="http://example.org/onto/class/yandex_mdb_mongodb_cluster"/>
    <rdfs:range rdf:resource="http://www.w3.org/2001/XMLSchema#string"/>
  </owl:DatatypeProperty>
  <owl:DatatypeProperty rdf:about="http://example.org/onto/prop/yandex_mdb_mongodb_cluster_compressors">
    <rdfs:label>compressors</rdfs:label>
    <rdfs:comment>Specifies the default compressor(s) to use for communication between this mongod or mongos. Accepts array of compressors. Order matters. Available compressors: snappy, zlib, zstd, disabled. To disable network compression, make `disabled` the only value. For more information, see the [net.Compression.Compressors](https://www.mongodb.com/docs/manual/reference/configuration-options/#mongodb-setting-net.compression.compressors) description in the official documentation.</rdfs:comment>
    <rdfs:domain rdf:resource="http://example.org/onto/class/yandex_mdb_mongodb_cluster"/>
    <rdfs:range rdf:resource="http://www.w3.org/2001/XMLSchema#string"/>
  </owl:DatatypeProperty>
  <owl:DatatypeProperty rdf:about="http://example.org/onto/prop/yandex_mdb_mongodb_cluster_max_incoming_connections">
    <rdfs:label>max_incoming_connections</rdfs:label>
    <rdfs:comment>The maximum number of simultaneous connections that host will accept. For more information, see the [net.maxIncomingConnections](https://www.mongodb.com/docs/manual/reference/configuration-options/#mongodb-setting-net.maxIncomingConnections) description in the official documentation.</rdfs:comment>
    <rdfs:domain rdf:resource="http://example.org/onto/class/yandex_mdb_mongodb_cluster"/>
    <rdfs:range rdf:resource="http://www.w3.org/2001/XMLSchema#string"/>
  </owl:DatatypeProperty>
  <owl:DatatypeProperty rdf:about="http://example.org/onto/prop/yandex_mdb_mongodb_cluster_mode">
    <rdfs:label>mode</rdfs:label>
    <rdfs:comment>Specifies which operations should be profiled. The following profiler levels are available: off, slow_op, all. For more information, see the [operationProfiling.mode](https://www.mongodb.com/docs/manual/reference/configuration-options/#mongodb-setting-operationProfiling.mode) description in the official documentation.</rdfs:comment>
    <rdfs:domain rdf:resource="http://example.org/onto/class/yandex_mdb_mongodb_cluster"/>
    <rdfs:range rdf:resource="http://www.w3.org/2001/XMLSchema#string"/>
  </owl:DatatypeProperty>
  <owl:DatatypeProperty rdf:about="http://example.org/onto/prop/yandex_mdb_mongodb_cluster_slow_op_sample_rate">
    <rdfs:label>slow_op_sample_rate</rdfs:label>
    <rdfs:comment>The fraction of slow operations that should be profiled or logged. Accepts values between 0 and 1, inclusive. For more information, see the [operationProfiling.slowOpSampleRate](https://www.mongodb.com/docs/manual/reference/configuration-options/#mongodb-setting-operationProfiling.slowOpSampleRate) description in the official documentation.</rdfs:comment>
    <rdfs:domain rdf:resource="http://example.org/onto/class/yandex_mdb_mongodb_cluster"/>
    <rdfs:range rdf:resource="http://www.w3.org/2001/XMLSchema#string"/>
  </owl:DatatypeProperty>
  <owl:DatatypeProperty rdf:about="http://example.org/onto/prop/yandex_mdb_mongodb_cluster_slow_op_threshold">
    <rdfs:label>slow_op_threshold</rdfs:label>
    <rdfs:comment>The slow operation time threshold, in milliseconds. Operations that run for longer than this threshold are considered slow. For more information, see the [operationProfiling.slowOpThresholdMs](https://www.mongodb.com/docs/manual/reference/configuration-options/#mongodb-setting-operationProfiling.slowOpThresholdMs) description in the official documentation.</rdfs:comment>
    <rdfs:domain rdf:resource="http://example.org/onto/class/yandex_mdb_mongodb_cluster"/>
    <rdfs:range rdf:resource="http://www.w3.org/2001/XMLSchema#string"/>
  </owl:DatatypeProperty>
  <owl:DatatypeProperty rdf:about="http://example.org/onto/prop/yandex_mdb_mongodb_cluster_enable_encryption">
    <rdfs:label>enable_encryption</rdfs:label>
    <rdfs:comment>Enables the encryption for the WiredTiger storage engine. Can be either true or false. For more information see [security.enableEncryption](https://www.mongodb.com/docs/manual/reference/configuration-options/#mongodb-setting-security.enableEncryption) description in the official documentation. Available only in enterprise edition.</rdfs:comment>
    <rdfs:domain rdf:resource="http://example.org/onto/class/yandex_mdb_mongodb_cluster"/>
    <rdfs:range rdf:resource="http://www.w3.org/2001/XMLSchema#string"/>
  </owl:DatatypeProperty>
  <owl:DatatypeProperty rdf:about="http://example.org/onto/prop/yandex_mdb_mongodb_cluster_client_certificate">
    <rdfs:label>client_certificate</rdfs:label>
    <rdfs:comment>String containing the client certificate used for authenticating MongoDB to the KMIP server. For more information see [security.kmip.clientCertificateFile](https://www.mongodb.com/docs/manual/reference/configuration-options/#mongodb-setting-security.kmip.clientCertificateFile) description in the official documentation.</rdfs:comment>
    <rdfs:domain rdf:resource="http://example.org/onto/class/yandex_mdb_mongodb_cluster"/>
    <rdfs:range rdf:resource="http://www.w3.org/2001/XMLSchema#string"/>
  </owl:DatatypeProperty>
  <owl:DatatypeProperty rdf:about="http://example.org/onto/prop/yandex_mdb_mongodb_cluster_key_identifier">
    <rdfs:label>key_identifier</rdfs:label>
    <rdfs:comment>Unique KMIP identifier for an existing key within the KMIP server. For more information see [security.kmip.keyIdentifier](https://www.mongodb.com/docs/manual/reference/configuration-options/#mongodb-setting-security.kmip.keyIdentifier) description in the official documentation.</rdfs:comment>
    <rdfs:domain rdf:resource="http://example.org/onto/class/yandex_mdb_mongodb_cluster"/>
    <rdfs:range rdf:resource="http://www.w3.org/2001/XMLSchema#string"/>
  </owl:DatatypeProperty>
  <owl:DatatypeProperty rdf:about="http://example.org/onto/prop/yandex_mdb_mongodb_cluster_port">
    <rdfs:label>port</rdfs:label>
    <rdfs:comment>Port number to use to communicate with the KMIP server. Default: 5696 For more information see [security.kmip.port](https://www.mongodb.com/docs/manual/reference/configuration-options/#mongodb-setting-security.kmip.port) description in the official documentation.</rdfs:comment>
    <rdfs:domain rdf:resource="http://example.org/onto/class/yandex_mdb_mongodb_cluster"/>
    <rdfs:range rdf:resource="http://www.w3.org/2001/XMLSchema#string"/>
  </owl:DatatypeProperty>
  <owl:DatatypeProperty rdf:about="http://example.org/onto/prop/yandex_mdb_mongodb_cluster_server_ca">
    <rdfs:label>server_ca</rdfs:label>
    <rdfs:comment>Path to CA File. Used for validating secure client connection to KMIP server. For more information see [security.kmip.serverCAFile](https://www.mongodb.com/docs/manual/reference/configuration-options/#mongodb-setting-security.kmip.serverCAFile) description in the official documentation.</rdfs:comment>
    <rdfs:domain rdf:resource="http://example.org/onto/class/yandex_mdb_mongodb_cluster"/>
    <rdfs:range rdf:resource="http://www.w3.org/2001/XMLSchema#string"/>
  </owl:DatatypeProperty>
  <owl:DatatypeProperty rdf:about="http://example.org/onto/prop/yandex_mdb_mongodb_cluster_server_name">
    <rdfs:label>server_name</rdfs:label>
    <rdfs:comment>Hostname or IP address of the KMIP server to connect to. For more information see [security.kmip.serverName](https://www.mongodb.com/docs/manual/reference/configuration-options/#mongodb-setting-security.kmip.serverName) description in the official documentation.</rdfs:comment>
    <rdfs:domain rdf:resource="http://example.org/onto/class/yandex_mdb_mongodb_cluster"/>
    <rdfs:range rdf:resource="http://www.w3.org/2001/XMLSchema#string"/>
  </owl:DatatypeProperty>
  <owl:DatatypeProperty rdf:about="http://example.org/onto/prop/yandex_mdb_mongodb_cluster_audit_authorization_success">
    <rdfs:label>audit_authorization_success</rdfs:label>
    <rdfs:comment>Enables the auditing of authorization successes. Can be either true or false. For more information, see the [auditAuthorizationSuccess](https://www.mongodb.com/docs/manual/reference/parameters/#mongodb-parameter-param.auditAuthorizationSuccess) description in the official documentation. Available only in enterprise edition.</rdfs:comment>
    <rdfs:domain rdf:resource="http://example.org/onto/class/yandex_mdb_mongodb_cluster"/>
    <rdfs:range rdf:resource="http://www.w3.org/2001/XMLSchema#string"/>
  </owl:DatatypeProperty>
  <owl:DatatypeProperty rdf:about="http://example.org/onto/prop/yandex_mdb_mongodb_cluster_enable_flow_control">
    <rdfs:label>enable_flow_control</rdfs:label>
    <rdfs:comment>Enables the flow control. Can be either true or false. For more information, see the [enableFlowControl](https://www.mongodb.com/docs/rapid/reference/parameters/#mongodb-parameter-param.enableFlowControl) description in the official documentation.</rdfs:comment>
    <rdfs:domain rdf:resource="http://example.org/onto/class/yandex_mdb_mongodb_cluster"/>
    <rdfs:range rdf:resource="http://www.w3.org/2001/XMLSchema#string"/>
  </owl:DatatypeProperty>
  <owl:DatatypeProperty rdf:about="http://example.org/onto/prop/yandex_mdb_mongodb_cluster_min_snapshot_history_window_in_seconds">
    <rdfs:label>min_snapshot_history_window_in_seconds</rdfs:label>
    <rdfs:comment>The minimum time window in seconds for which the storage engine keeps the snapshot history. For more information, see the [minSnapshotHistoryWindowInSeconds](https://www.mongodb.com/docs/manual/reference/parameters/#mongodb-parameter-param.minSnapshotHistoryWindowInSeconds) description in the official documentation.</rdfs:comment>
    <rdfs:domain rdf:resource="http://example.org/onto/class/yandex_mdb_mongodb_cluster"/>
    <rdfs:range rdf:resource="http://www.w3.org/2001/XMLSchema#string"/>
  </owl:DatatypeProperty>
  <owl:DatatypeProperty rdf:about="http://example.org/onto/prop/yandex_mdb_mongodb_cluster_commit_interval">
    <rdfs:label>commit_interval</rdfs:label>
    <rdfs:comment>The maximum amount of time in milliseconds that the mongod process allows between journal operations. For more information, see the [storage.journal.commitIntervalMs](https://www.mongodb.com/docs/manual/reference/configuration-options/#mongodb-setting-storage.journal.commitIntervalMs) description in the official documentation.</rdfs:comment>
    <rdfs:domain rdf:resource="http://example.org/onto/class/yandex_mdb_mongodb_cluster"/>
    <rdfs:range rdf:resource="http://www.w3.org/2001/XMLSchema#string"/>
  </owl:DatatypeProperty>
  <owl:DatatypeProperty rdf:about="http://example.org/onto/prop/yandex_mdb_mongodb_cluster_block_compressor">
    <rdfs:label>block_compressor</rdfs:label>
    <rdfs:comment>Specifies the default compression for collection data. You can override this on a per-collection basis when creating collections. Available compressors are: none, snappy, zlib, zstd. This setting available only on `mongod` hosts. For more information, see the [storage.wiredTiger.collectionConfig.blockCompressor](https://www.mongodb.com/docs/manual/reference/configuration-options/#mongodb-setting-storage.wiredTiger.collectionConfig.blockCompressor) description in the official documentation.</rdfs:comment>
    <rdfs:domain rdf:resource="http://example.org/onto/class/yandex_mdb_mongodb_cluster"/>
    <rdfs:range rdf:resource="http://www.w3.org/2001/XMLSchema#string"/>
  </owl:DatatypeProperty>
  <owl:DatatypeProperty rdf:about="http://example.org/onto/prop/yandex_mdb_mongodb_cluster_cache_size_gb">
    <rdfs:label>cache_size_gb</rdfs:label>
    <rdfs:comment>Defines the maximum size of the internal cache that WiredTiger will use for all data. For more information, see the [storage.wiredTiger.engineConfig.cacheSizeGB](https://www.mongodb.com/docs/manual/reference/configuration-options/#mongodb-setting-storage.wiredTiger.engineConfig.cacheSizeGB) description in the official documentation.</rdfs:comment>
    <rdfs:domain rdf:resource="http://example.org/onto/class/yandex_mdb_mongodb_cluster"/>
    <rdfs:range rdf:resource="http://www.w3.org/2001/XMLSchema#string"/>
  </owl:DatatypeProperty>
  <owl:DatatypeProperty rdf:about="http://example.org/onto/prop/yandex_mdb_mongodb_cluster_prefix_compression">
    <rdfs:label>prefix_compression</rdfs:label>
    <rdfs:comment>Enables or disables prefix compression for index data. Ð¡an be either true or false. For more information, see the [storage.wiredTiger.indexConfig.prefixCompression](https://www.mongodb.com/docs/manual/reference/configuration-options/#mongodb-setting-storage.wiredTiger.indexConfig.prefixCompression) description in the official documentation.</rdfs:comment>
    <rdfs:domain rdf:resource="http://example.org/onto/class/yandex_mdb_mongodb_cluster"/>
    <rdfs:range rdf:resource="http://www.w3.org/2001/XMLSchema#string"/>
  </owl:DatatypeProperty>
  <owl:DatatypeProperty rdf:about="http://example.org/onto/prop/yandex_mdb_mongodb_cluster_compressors">
    <rdfs:label>compressors</rdfs:label>
    <rdfs:comment>Specifies the default compressor(s) to use for communication between this mongod or mongos. Accepts array of compressors. Order matters. Available compressors: snappy, zlib, zstd, disabled. To disable network compression, make `disabled` the only value. For more information, see the [net.Compression.Compressors](https://www.mongodb.com/docs/manual/reference/configuration-options/#mongodb-setting-net.compression.compressors) description in the official documentation.</rdfs:comment>
    <rdfs:domain rdf:resource="http://example.org/onto/class/yandex_mdb_mongodb_cluster"/>
    <rdfs:range rdf:resource="http://www.w3.org/2001/XMLSchema#string"/>
  </owl:DatatypeProperty>
  <owl:DatatypeProperty rdf:about="http://example.org/onto/prop/yandex_mdb_mongodb_cluster_max_incoming_connections">
    <rdfs:label>max_incoming_connections</rdfs:label>
    <rdfs:comment>The maximum number of simultaneous connections that host will accept. For more information, see the [net.maxIncomingConnections](https://www.mongodb.com/docs/manual/reference/configuration-options/#mongodb-setting-net.maxIncomingConnections) description in the official documentation.</rdfs:comment>
    <rdfs:domain rdf:resource="http://example.org/onto/class/yandex_mdb_mongodb_cluster"/>
    <rdfs:range rdf:resource="http://www.w3.org/2001/XMLSchema#string"/>
  </owl:DatatypeProperty>
  <owl:DatatypeProperty rdf:about="http://example.org/onto/prop/yandex_mdb_mongodb_cluster_enabled">
    <rdfs:label>enabled</rdfs:label>
    <rdfs:comment>Enable or disable performance diagnostics.</rdfs:comment>
    <rdfs:domain rdf:resource="http://example.org/onto/class/yandex_mdb_mongodb_cluster"/>
    <rdfs:range rdf:resource="http://www.w3.org/2001/XMLSchema#string"/>
  </owl:DatatypeProperty>
  <owl:DatatypeProperty rdf:about="http://example.org/onto/prop/yandex_mdb_mongodb_cluster_name">
    <rdfs:label>name</rdfs:label>
    <rdfs:comment>The name of the database.</rdfs:comment>
    <rdfs:domain rdf:resource="http://example.org/onto/class/yandex_mdb_mongodb_cluster"/>
    <rdfs:range rdf:resource="http://www.w3.org/2001/XMLSchema#string"/>
  </owl:DatatypeProperty>
  <owl:DatatypeProperty rdf:about="http://example.org/onto/prop/yandex_mdb_mongodb_cluster_disk_size_limit">
    <rdfs:label>disk_size_limit</rdfs:label>
    <rdfs:comment>Limit of disk size after autoscaling (GiB).</rdfs:comment>
    <rdfs:domain rdf:resource="http://example.org/onto/class/yandex_mdb_mongodb_cluster"/>
    <rdfs:range rdf:resource="http://www.w3.org/2001/XMLSchema#string"/>
  </owl:DatatypeProperty>
  <owl:DatatypeProperty rdf:about="http://example.org/onto/prop/yandex_mdb_mongodb_cluster_emergency_usage_threshold">
    <rdfs:label>emergency_usage_threshold</rdfs:label>
    <rdfs:comment>Immediate autoscaling disk usage (percent).</rdfs:comment>
    <rdfs:domain rdf:resource="http://example.org/onto/class/yandex_mdb_mongodb_cluster"/>
    <rdfs:range rdf:resource="http://www.w3.org/2001/XMLSchema#string"/>
  </owl:DatatypeProperty>
  <owl:DatatypeProperty rdf:about="http://example.org/onto/prop/yandex_mdb_mongodb_cluster_planned_usage_threshold">
    <rdfs:label>planned_usage_threshold</rdfs:label>
    <rdfs:comment>Maintenance window autoscaling disk usage (percent).</rdfs:comment>
    <rdfs:domain rdf:resource="http://example.org/onto/class/yandex_mdb_mongodb_cluster"/>
    <rdfs:range rdf:resource="http://www.w3.org/2001/XMLSchema#string"/>
  </owl:DatatypeProperty>
  <owl:DatatypeProperty rdf:about="http://example.org/onto/prop/yandex_mdb_mongodb_cluster_disk_size_limit">
    <rdfs:label>disk_size_limit</rdfs:label>
    <rdfs:comment>Limit of disk size after autoscaling (GiB).</rdfs:comment>
    <rdfs:domain rdf:resource="http://example.org/onto/class/yandex_mdb_mongodb_cluster"/>
    <rdfs:range rdf:resource="http://www.w3.org/2001/XMLSchema#string"/>
  </owl:DatatypeProperty>
  <owl:DatatypeProperty rdf:about="http://example.org/onto/prop/yandex_mdb_mongodb_cluster_emergency_usage_threshold">
    <rdfs:label>emergency_usage_threshold</rdfs:label>
    <rdfs:comment>Immediate autoscaling disk usage (percent).</rdfs:comment>
    <rdfs:domain rdf:resource="http://example.org/onto/class/yandex_mdb_mongodb_cluster"/>
    <rdfs:range rdf:resource="http://www.w3.org/2001/XMLSchema#string"/>
  </owl:DatatypeProperty>
  <owl:DatatypeProperty rdf:about="http://example.org/onto/prop/yandex_mdb_mongodb_cluster_planned_usage_threshold">
    <rdfs:label>planned_usage_threshold</rdfs:label>
    <rdfs:comment>Maintenance window autoscaling disk usage (percent).</rdfs:comment>
    <rdfs:domain rdf:resource="http://example.org/onto/class/yandex_mdb_mongodb_cluster"/>
    <rdfs:range rdf:resource="http://www.w3.org/2001/XMLSchema#string"/>
  </owl:DatatypeProperty>
  <owl:DatatypeProperty rdf:about="http://example.org/onto/prop/yandex_mdb_mongodb_cluster_disk_size_limit">
    <rdfs:label>disk_size_limit</rdfs:label>
    <rdfs:comment>Limit of disk size after autoscaling (GiB).</rdfs:comment>
    <rdfs:domain rdf:resource="http://example.org/onto/class/yandex_mdb_mongodb_cluster"/>
    <rdfs:range rdf:resource="http://www.w3.org/2001/XMLSchema#string"/>
  </owl:DatatypeProperty>
  <owl:DatatypeProperty rdf:about="http://example.org/onto/prop/yandex_mdb_mongodb_cluster_emergency_usage_threshold">
    <rdfs:label>emergency_usage_threshold</rdfs:label>
    <rdfs:comment>Immediate autoscaling disk usage (percent).</rdfs:comment>
    <rdfs:domain rdf:resource="http://example.org/onto/class/yandex_mdb_mongodb_cluster"/>
    <rdfs:range rdf:resource="http://www.w3.org/2001/XMLSchema#string"/>
  </owl:DatatypeProperty>
  <owl:DatatypeProperty rdf:about="http://example.org/onto/prop/yandex_mdb_mongodb_cluster_planned_usage_threshold">
    <rdfs:label>planned_usage_threshold</rdfs:label>
    <rdfs:comment>Maintenance window autoscaling disk usage (percent).</rdfs:comment>
    <rdfs:domain rdf:resource="http://example.org/onto/class/yandex_mdb_mongodb_cluster"/>
    <rdfs:range rdf:resource="http://www.w3.org/2001/XMLSchema#string"/>
  </owl:DatatypeProperty>
  <owl:DatatypeProperty rdf:about="http://example.org/onto/prop/yandex_mdb_mongodb_cluster_disk_size_limit">
    <rdfs:label>disk_size_limit</rdfs:label>
    <rdfs:comment>Limit of disk size after autoscaling (GiB).</rdfs:comment>
    <rdfs:domain rdf:resource="http://example.org/onto/class/yandex_mdb_mongodb_cluster"/>
    <rdfs:range rdf:resource="http://www.w3.org/2001/XMLSchema#string"/>
  </owl:DatatypeProperty>
  <owl:DatatypeProperty rdf:about="http://example.org/onto/prop/yandex_mdb_mongodb_cluster_emergency_usage_threshold">
    <rdfs:label>emergency_usage_threshold</rdfs:label>
    <rdfs:comment>Immediate autoscaling disk usage (percent).</rdfs:comment>
    <rdfs:domain rdf:resource="http://example.org/onto/class/yandex_mdb_mongodb_cluster"/>
    <rdfs:range rdf:resource="http://www.w3.org/2001/XMLSchema#string"/>
  </owl:DatatypeProperty>
  <owl:DatatypeProperty rdf:about="http://example.org/onto/prop/yandex_mdb_mongodb_cluster_planned_usage_threshold">
    <rdfs:label>planned_usage_threshold</rdfs:label>
    <rdfs:comment>Maintenance window autoscaling disk usage (percent).</rdfs:comment>
    <rdfs:domain rdf:resource="http://example.org/onto/class/yandex_mdb_mongodb_cluster"/>
    <rdfs:range rdf:resource="http://www.w3.org/2001/XMLSchema#string"/>
  </owl:DatatypeProperty>
  <owl:DatatypeProperty rdf:about="http://example.org/onto/prop/yandex_mdb_mongodb_cluster_assign_public_ip">
    <rdfs:label>assign_public_ip</rdfs:label>
    <rdfs:comment>Should this host have assigned public IP assigned. Can be either `true` or `false`.</rdfs:comment>
    <rdfs:domain rdf:resource="http://example.org/onto/class/yandex_mdb_mongodb_cluster"/>
    <rdfs:range rdf:resource="http://www.w3.org/2001/XMLSchema#string"/>
  </owl:DatatypeProperty>
  <owl:DatatypeProperty rdf:about="http://example.org/onto/prop/yandex_mdb_mongodb_cluster_health">
    <rdfs:label>health</rdfs:label>
    <rdfs:comment>The health of the host.</rdfs:comment>
    <rdfs:domain rdf:resource="http://example.org/onto/class/yandex_mdb_mongodb_cluster"/>
    <rdfs:range rdf:resource="http://www.w3.org/2001/XMLSchema#string"/>
  </owl:DatatypeProperty>
  <owl:DatatypeProperty rdf:about="http://example.org/onto/prop/yandex_mdb_mongodb_cluster_name">
    <rdfs:label>name</rdfs:label>
    <rdfs:comment>The fully qualified domain name of the host. Computed on server side.</rdfs:comment>
    <rdfs:domain rdf:resource="http://example.org/onto/class/yandex_mdb_mongodb_cluster"/>
    <rdfs:range rdf:resource="http://www.w3.org/2001/XMLSchema#string"/>
  </owl:DatatypeProperty>
  <owl:DatatypeProperty rdf:about="http://example.org/onto/prop/yandex_mdb_mongodb_cluster_role">
    <rdfs:label>role</rdfs:label>
    <rdfs:comment>The role of the cluster (either PRIMARY or SECONDARY).</rdfs:comment>
    <rdfs:domain rdf:resource="http://example.org/onto/class/yandex_mdb_mongodb_cluster"/>
    <rdfs:range rdf:resource="http://www.w3.org/2001/XMLSchema#string"/>
  </owl:DatatypeProperty>
  <owl:DatatypeProperty rdf:about="http://example.org/onto/prop/yandex_mdb_mongodb_cluster_shard_name">
    <rdfs:label>shard_name</rdfs:label>
    <rdfs:comment>The name of the shard to which the host belongs. Only for sharded cluster.</rdfs:comment>
    <rdfs:domain rdf:resource="http://example.org/onto/class/yandex_mdb_mongodb_cluster"/>
    <rdfs:range rdf:resource="http://www.w3.org/2001/XMLSchema#string"/>
  </owl:DatatypeProperty>
  <owl:DatatypeProperty rdf:about="http://example.org/onto/prop/yandex_mdb_mongodb_cluster_subnet_id">
    <rdfs:label>subnet_id</rdfs:label>
    <rdfs:comment>The ID of the subnet, to which the host belongs. The subnet must be a part of the network to which the cluster belongs.</rdfs:comment>
    <rdfs:domain rdf:resource="http://example.org/onto/class/yandex_mdb_mongodb_cluster"/>
    <rdfs:range rdf:resource="http://www.w3.org/2001/XMLSchema#string"/>
  </owl:DatatypeProperty>
  <owl:DatatypeProperty rdf:about="http://example.org/onto/prop/yandex_mdb_mongodb_cluster_type">
    <rdfs:label>type</rdfs:label>
    <rdfs:comment>Type of Mongo daemon which runs on this host (mongod, mongos, mongocfg, mongoinfra). Defaults to `mongod`.</rdfs:comment>
    <rdfs:domain rdf:resource="http://example.org/onto/class/yandex_mdb_mongodb_cluster"/>
    <rdfs:range rdf:resource="http://www.w3.org/2001/XMLSchema#string"/>
  </owl:DatatypeProperty>
  <owl:DatatypeProperty rdf:about="http://example.org/onto/prop/yandex_mdb_mongodb_cluster_zone_id">
    <rdfs:label>zone_id</rdfs:label>
    <rdfs:comment>The [availability zone](https://yandex.cloud/docs/overview/concepts/geo-scope) where resource is located. If it is not provided, the default provider zone will be used.</rdfs:comment>
    <rdfs:domain rdf:resource="http://example.org/onto/class/yandex_mdb_mongodb_cluster"/>
    <rdfs:range rdf:resource="http://www.w3.org/2001/XMLSchema#string"/>
  </owl:DatatypeProperty>
  <owl:DatatypeProperty rdf:about="http://example.org/onto/prop/yandex_mdb_mongodb_cluster_hidden">
    <rdfs:label>hidden</rdfs:label>
    <rdfs:comment>Should this host be hidden in replicaset. Can be either `true` of `false`. For more information see [the official documentation](https://www.mongodb.com/docs/current/reference/replica-configuration/#mongodb-rsconf-rsconf.members-n-.hidden).</rdfs:comment>
    <rdfs:domain rdf:resource="http://example.org/onto/class/yandex_mdb_mongodb_cluster"/>
    <rdfs:range rdf:resource="http://www.w3.org/2001/XMLSchema#string"/>
  </owl:DatatypeProperty>
  <owl:DatatypeProperty rdf:about="http://example.org/onto/prop/yandex_mdb_mongodb_cluster_priority">
    <rdfs:label>priority</rdfs:label>
    <rdfs:comment>A floating point number that indicates the relative likelihood of a replica set member to become the primary. For more information see [the official documentation](https://www.mongodb.com/docs/current/reference/replica-configuration/#mongodb-rsconf-rsconf.members-n-.priority).</rdfs:comment>
    <rdfs:domain rdf:resource="http://example.org/onto/class/yandex_mdb_mongodb_cluster"/>
    <rdfs:range rdf:resource="http://www.w3.org/2001/XMLSchema#string"/>
  </owl:DatatypeProperty>
  <owl:DatatypeProperty rdf:about="http://example.org/onto/prop/yandex_mdb_mongodb_cluster_secondary_delay_secs">
    <rdfs:label>secondary_delay_secs</rdfs:label>
    <rdfs:comment>The number of seconds `behind` the primary that this replica set member should `lag`. For more information see [the official documentation](https://www.mongodb.com/docs/current/reference/replica-configuration/#mongodb-rsconf-rsconf.members-n-.secondaryDelaySecs).</rdfs:comment>
    <rdfs:domain rdf:resource="http://example.org/onto/class/yandex_mdb_mongodb_cluster"/>
    <rdfs:range rdf:resource="http://www.w3.org/2001/XMLSchema#string"/>
  </owl:DatatypeProperty>
  <owl:DatatypeProperty rdf:about="http://example.org/onto/prop/yandex_mdb_mongodb_cluster_tags">
    <rdfs:label>tags</rdfs:label>
    <rdfs:comment>A set of key/value pairs to assign for the replica set member. For more information see [the official documentation](https://www.mongodb.com/docs/current/reference/replica-configuration/#mongodb-rsconf-rsconf.members-n-.tags).</rdfs:comment>
    <rdfs:domain rdf:resource="http://example.org/onto/class/yandex_mdb_mongodb_cluster"/>
    <rdfs:range rdf:resource="http://www.w3.org/2001/XMLSchema#string"/>
  </owl:DatatypeProperty>
  <owl:DatatypeProperty rdf:about="http://example.org/onto/prop/yandex_mdb_mongodb_cluster_day">
    <rdfs:label>day</rdfs:label>
    <rdfs:comment>Day of week for maintenance window if window type is weekly. Possible values: `MON`, `TUE`, `WED`, `THU`, `FRI`, `SAT`, `SUN`.</rdfs:comment>
    <rdfs:domain rdf:resource="http://example.org/onto/class/yandex_mdb_mongodb_cluster"/>
    <rdfs:range rdf:resource="http://www.w3.org/2001/XMLSchema#string"/>
  </owl:DatatypeProperty>
  <owl:DatatypeProperty rdf:about="http://example.org/onto/prop/yandex_mdb_mongodb_cluster_hour">
    <rdfs:label>hour</rdfs:label>
    <rdfs:comment>Hour of day in UTC time zone (1-24) for maintenance window if window type is weekly.</rdfs:comment>
    <rdfs:domain rdf:resource="http://example.org/onto/class/yandex_mdb_mongodb_cluster"/>
    <rdfs:range rdf:resource="http://www.w3.org/2001/XMLSchema#string"/>
  </owl:DatatypeProperty>
  <owl:DatatypeProperty rdf:about="http://example.org/onto/prop/yandex_mdb_mongodb_cluster_type">
    <rdfs:label>type</rdfs:label>
    <rdfs:comment>Type of maintenance window. Can be either `ANYTIME` or `WEEKLY`. A day and hour of window need to be specified with weekly window.</rdfs:comment>
    <rdfs:domain rdf:resource="http://example.org/onto/class/yandex_mdb_mongodb_cluster"/>
    <rdfs:range rdf:resource="http://www.w3.org/2001/XMLSchema#string"/>
  </owl:DatatypeProperty>
  <owl:DatatypeProperty rdf:about="http://example.org/onto/prop/yandex_mdb_mongodb_cluster_disk_size">
    <rdfs:label>disk_size</rdfs:label>
    <rdfs:comment>Volume of the storage available to a MongoDB host, in gigabytes.</rdfs:comment>
    <rdfs:domain rdf:resource="http://example.org/onto/class/yandex_mdb_mongodb_cluster"/>
    <rdfs:range rdf:resource="http://www.w3.org/2001/XMLSchema#string"/>
  </owl:DatatypeProperty>
  <owl:DatatypeProperty rdf:about="http://example.org/onto/prop/yandex_mdb_mongodb_cluster_disk_type_id">
    <rdfs:label>disk_type_id</rdfs:label>
    <rdfs:comment>Type of the storage of MongoDB hosts. For more information see [the official documentation](https://yandex.cloud/docs/managed-clickhouse/concepts/storage).</rdfs:comment>
    <rdfs:domain rdf:resource="http://example.org/onto/class/yandex_mdb_mongodb_cluster"/>
    <rdfs:range rdf:resource="http://www.w3.org/2001/XMLSchema#string"/>
  </owl:DatatypeProperty>
  <owl:DatatypeProperty rdf:about="http://example.org/onto/prop/yandex_mdb_mongodb_cluster_resource_preset_id">
    <rdfs:label>resource_preset_id</rdfs:label>
    <rdfs:comment>The ID of the preset for computational resources available to a MongoDB host (CPU, memory etc.). For more information, see [the official documentation](https://yandex.cloud/docs/managed-mongodb/concepts).</rdfs:comment>
    <rdfs:domain rdf:resource="http://example.org/onto/class/yandex_mdb_mongodb_cluster"/>
    <rdfs:range rdf:resource="http://www.w3.org/2001/XMLSchema#string"/>
  </owl:DatatypeProperty>
  <owl:DatatypeProperty rdf:about="http://example.org/onto/prop/yandex_mdb_mongodb_cluster_disk_size">
    <rdfs:label>disk_size</rdfs:label>
    <rdfs:comment>Volume of the storage available to a MongoDB host, in gigabytes.</rdfs:comment>
    <rdfs:domain rdf:resource="http://example.org/onto/class/yandex_mdb_mongodb_cluster"/>
    <rdfs:range rdf:resource="http://www.w3.org/2001/XMLSchema#string"/>
  </owl:DatatypeProperty>
  <owl:DatatypeProperty rdf:about="http://example.org/onto/prop/yandex_mdb_mongodb_cluster_disk_type_id">
    <rdfs:label>disk_type_id</rdfs:label>
    <rdfs:comment>Type of the storage of MongoDB hosts. For more information see [the official documentation](https://yandex.cloud/docs/managed-clickhouse/concepts/storage).</rdfs:comment>
    <rdfs:domain rdf:resource="http://example.org/onto/class/yandex_mdb_mongodb_cluster"/>
    <rdfs:range rdf:resource="http://www.w3.org/2001/XMLSchema#string"/>
  </owl:DatatypeProperty>
  <owl:DatatypeProperty rdf:about="http://example.org/onto/prop/yandex_mdb_mongodb_cluster_resource_preset_id">
    <rdfs:label>resource_preset_id</rdfs:label>
    <rdfs:comment>The ID of the preset for computational resources available to a MongoDB host (CPU, memory etc.). For more information, see [the official documentation](https://yandex.cloud/docs/managed-mongodb/concepts).</rdfs:comment>
    <rdfs:domain rdf:resource="http://example.org/onto/class/yandex_mdb_mongodb_cluster"/>
    <rdfs:range rdf:resource="http://www.w3.org/2001/XMLSchema#string"/>
  </owl:DatatypeProperty>
  <owl:DatatypeProperty rdf:about="http://example.org/onto/prop/yandex_mdb_mongodb_cluster_disk_size">
    <rdfs:label>disk_size</rdfs:label>
    <rdfs:comment>Volume of the storage available to a MongoDB host, in gigabytes.</rdfs:comment>
    <rdfs:domain rdf:resource="http://example.org/onto/class/yandex_mdb_mongodb_cluster"/>
    <rdfs:range rdf:resource="http://www.w3.org/2001/XMLSchema#string"/>
  </owl:DatatypeProperty>
  <owl:DatatypeProperty rdf:about="http://example.org/onto/prop/yandex_mdb_mongodb_cluster_disk_type_id">
    <rdfs:label>disk_type_id</rdfs:label>
    <rdfs:comment>Type of the storage of MongoDB hosts. For more information see [the official documentation](https://yandex.cloud/docs/managed-clickhouse/concepts/storage).</rdfs:comment>
    <rdfs:domain rdf:resource="http://example.org/onto/class/yandex_mdb_mongodb_cluster"/>
    <rdfs:range rdf:resource="http://www.w3.org/2001/XMLSchema#string"/>
  </owl:DatatypeProperty>
  <owl:DatatypeProperty rdf:about="http://example.org/onto/prop/yandex_mdb_mongodb_cluster_resource_preset_id">
    <rdfs:label>resource_preset_id</rdfs:label>
    <rdfs:comment>The ID of the preset for computational resources available to a MongoDB host (CPU, memory etc.). For more information, see [the official documentation](https://yandex.cloud/docs/managed-mongodb/concepts).</rdfs:comment>
    <rdfs:domain rdf:resource="http://example.org/onto/class/yandex_mdb_mongodb_cluster"/>
    <rdfs:range rdf:resource="http://www.w3.org/2001/XMLSchema#string"/>
  </owl:DatatypeProperty>
  <owl:DatatypeProperty rdf:about="http://example.org/onto/prop/yandex_mdb_mongodb_cluster_disk_size">
    <rdfs:label>disk_size</rdfs:label>
    <rdfs:comment>Volume of the storage available to a MongoDB host, in gigabytes.</rdfs:comment>
    <rdfs:domain rdf:resource="http://example.org/onto/class/yandex_mdb_mongodb_cluster"/>
    <rdfs:range rdf:resource="http://www.w3.org/2001/XMLSchema#string"/>
  </owl:DatatypeProperty>
  <owl:DatatypeProperty rdf:about="http://example.org/onto/prop/yandex_mdb_mongodb_cluster_disk_type_id">
    <rdfs:label>disk_type_id</rdfs:label>
    <rdfs:comment>Type of the storage of MongoDB hosts. For more information see [the official documentation](https://yandex.cloud/docs/managed-clickhouse/concepts/storage).</rdfs:comment>
    <rdfs:domain rdf:resource="http://example.org/onto/class/yandex_mdb_mongodb_cluster"/>
    <rdfs:range rdf:resource="http://www.w3.org/2001/XMLSchema#string"/>
  </owl:DatatypeProperty>
  <owl:DatatypeProperty rdf:about="http://example.org/onto/prop/yandex_mdb_mongodb_cluster_resource_preset_id">
    <rdfs:label>resource_preset_id</rdfs:label>
    <rdfs:comment>The ID of the preset for computational resources available to a MongoDB host (CPU, memory etc.). For more information, see [the official documentation](https://yandex.cloud/docs/managed-mongodb/concepts).</rdfs:comment>
    <rdfs:domain rdf:resource="http://example.org/onto/class/yandex_mdb_mongodb_cluster"/>
    <rdfs:range rdf:resource="http://www.w3.org/2001/XMLSchema#string"/>
  </owl:DatatypeProperty>
  <owl:DatatypeProperty rdf:about="http://example.org/onto/prop/yandex_mdb_mongodb_cluster_disk_size">
    <rdfs:label>disk_size</rdfs:label>
    <rdfs:comment>Volume of the storage available to a MongoDB host, in gigabytes.</rdfs:comment>
    <rdfs:domain rdf:resource="http://example.org/onto/class/yandex_mdb_mongodb_cluster"/>
    <rdfs:range rdf:resource="http://www.w3.org/2001/XMLSchema#string"/>
  </owl:DatatypeProperty>
  <owl:DatatypeProperty rdf:about="http://example.org/onto/prop/yandex_mdb_mongodb_cluster_disk_type_id">
    <rdfs:label>disk_type_id</rdfs:label>
    <rdfs:comment>Type of the storage of MongoDB hosts. For more information see [the official documentation](https://yandex.cloud/docs/managed-clickhouse/concepts/storage).</rdfs:comment>
    <rdfs:domain rdf:resource="http://example.org/onto/class/yandex_mdb_mongodb_cluster"/>
    <rdfs:range rdf:resource="http://www.w3.org/2001/XMLSchema#string"/>
  </owl:DatatypeProperty>
  <owl:DatatypeProperty rdf:about="http://example.org/onto/prop/yandex_mdb_mongodb_cluster_resource_preset_id">
    <rdfs:label>resource_preset_id</rdfs:label>
    <rdfs:comment>The ID of the preset for computational resources available to a MongoDB host (CPU, memory etc.). For more information, see [the official documentation](https://yandex.cloud/docs/managed-mongodb/concepts).</rdfs:comment>
    <rdfs:domain rdf:resource="http://example.org/onto/class/yandex_mdb_mongodb_cluster"/>
    <rdfs:range rdf:resource="http://www.w3.org/2001/XMLSchema#string"/>
  </owl:DatatypeProperty>
  <owl:DatatypeProperty rdf:about="http://example.org/onto/prop/yandex_mdb_mongodb_cluster_backup_id">
    <rdfs:label>backup_id</rdfs:label>
    <rdfs:comment>Backup ID. The cluster will be created from the specified backup. [How to get a list of PostgreSQL backups](https://yandex.cloud/docs/managed-mongodb/operations/cluster-backups).</rdfs:comment>
    <rdfs:domain rdf:resource="http://example.org/onto/class/yandex_mdb_mongodb_cluster"/>
    <rdfs:range rdf:resource="http://www.w3.org/2001/XMLSchema#string"/>
  </owl:DatatypeProperty>
  <owl:DatatypeProperty rdf:about="http://example.org/onto/prop/yandex_mdb_mongodb_cluster_time">
    <rdfs:label>time</rdfs:label>
    <rdfs:comment>Timestamp of the moment to which the MongoDB cluster should be restored. (Format: `2006-01-02T15:04:05` - UTC). When not set, current time is used.</rdfs:comment>
    <rdfs:domain rdf:resource="http://example.org/onto/class/yandex_mdb_mongodb_cluster"/>
    <rdfs:range rdf:resource="http://www.w3.org/2001/XMLSchema#string"/>
  </owl:DatatypeProperty>
  <owl:DatatypeProperty rdf:about="http://example.org/onto/prop/yandex_mdb_mongodb_cluster_create">
    <rdfs:label>create</rdfs:label>
    <rdfs:domain rdf:resource="http://example.org/onto/class/yandex_mdb_mongodb_cluster"/>
    <rdfs:range rdf:resource="http://www.w3.org/2001/XMLSchema#string"/>
  </owl:DatatypeProperty>
  <owl:DatatypeProperty rdf:about="http://example.org/onto/prop/yandex_mdb_mongodb_cluster_delete">
    <rdfs:label>delete</rdfs:label>
    <rdfs:domain rdf:resource="http://example.org/onto/class/yandex_mdb_mongodb_cluster"/>
    <rdfs:range rdf:resource="http://www.w3.org/2001/XMLSchema#string"/>
  </owl:DatatypeProperty>
  <owl:DatatypeProperty rdf:about="http://example.org/onto/prop/yandex_mdb_mongodb_cluster_update">
    <rdfs:label>update</rdfs:label>
    <rdfs:domain rdf:resource="http://example.org/onto/class/yandex_mdb_mongodb_cluster"/>
    <rdfs:range rdf:resource="http://www.w3.org/2001/XMLSchema#string"/>
  </owl:DatatypeProperty>
  <owl:DatatypeProperty rdf:about="http://example.org/onto/prop/yandex_mdb_mongodb_cluster_name">
    <rdfs:label>name</rdfs:label>
    <rdfs:comment>The name of the user.</rdfs:comment>
    <rdfs:domain rdf:resource="http://example.org/onto/class/yandex_mdb_mongodb_cluster"/>
    <rdfs:range rdf:resource="http://www.w3.org/2001/XMLSchema#string"/>
  </owl:DatatypeProperty>
  <owl:DatatypeProperty rdf:about="http://example.org/onto/prop/yandex_mdb_mongodb_cluster_password">
    <rdfs:label>password</rdfs:label>
    <rdfs:comment>The password of the user.</rdfs:comment>
    <rdfs:domain rdf:resource="http://example.org/onto/class/yandex_mdb_mongodb_cluster"/>
    <rdfs:range rdf:resource="http://www.w3.org/2001/XMLSchema#string"/>
  </owl:DatatypeProperty>
  <owl:DatatypeProperty rdf:about="http://example.org/onto/prop/yandex_mdb_mongodb_cluster_database_name">
    <rdfs:label>database_name</rdfs:label>
    <rdfs:comment>The name of the database that the permission grants access to.</rdfs:comment>
    <rdfs:domain rdf:resource="http://example.org/onto/class/yandex_mdb_mongodb_cluster"/>
    <rdfs:range rdf:resource="http://www.w3.org/2001/XMLSchema#string"/>
  </owl:DatatypeProperty>
  <owl:DatatypeProperty rdf:about="http://example.org/onto/prop/yandex_mdb_mongodb_cluster_roles">
    <rdfs:label>roles</rdfs:label>
    <rdfs:comment>The roles of the user in this database. For more information see [the official documentation](https://yandex.cloud/docs/managed-mongodb/concepts/users-and-roles).</rdfs:comment>
    <rdfs:domain rdf:resource="http://example.org/onto/class/yandex_mdb_mongodb_cluster"/>
    <rdfs:range rdf:resource="http://www.w3.org/2001/XMLSchema#string"/>
  </owl:DatatypeProperty>
</rdf:RDF>
