<?xml version="1.0" encoding="UTF-8"?>
<rdf:RDF
  xmlns:rdf="http://www.w3.org/1999/02/22-rdf-syntax-ns#"
  xmlns:rdfs="http://www.w3.org/2000/01/rdf-schema#"
  xmlns:owl="http://www.w3.org/2002/07/owl#"
  xmlns:xsd="http://www.w3.org/2001/XMLSchema#"
  xml:base="http://example.org/onto/">
  <owl:Class rdf:about="http://example.org/onto/class/yandex_compute_gpu_cluster">
    <rdfs:label>yandex_compute_gpu_cluster</rdfs:label>
    <rdfs:comment>A GPU cluster. For details about the concept, see [documentation](/docs/compute/concepts/gpus#gpu-clusters).</rdfs:comment>
  </owl:Class>
  <owl:DatatypeProperty rdf:about="http://example.org/onto/prop/yandex_compute_gpu_cluster_created_at">
    <rdfs:label>created_at</rdfs:label>
    <rdfs:comment>Creation timestamp.</rdfs:comment>
    <rdfs:domain rdf:resource="http://example.org/onto/class/yandex_compute_gpu_cluster"/>
    <rdfs:range rdf:resource="http://www.w3.org/2001/XMLSchema#string"/>
  </owl:DatatypeProperty>
  <owl:DatatypeProperty rdf:about="http://example.org/onto/prop/yandex_compute_gpu_cluster_description">
    <rdfs:label>description</rdfs:label>
    <rdfs:comment>Description of the GPU cluster.</rdfs:comment>
    <rdfs:domain rdf:resource="http://example.org/onto/class/yandex_compute_gpu_cluster"/>
    <rdfs:range rdf:resource="http://www.w3.org/2001/XMLSchema#string"/>
  </owl:DatatypeProperty>
  <owl:DatatypeProperty rdf:about="http://example.org/onto/prop/yandex_compute_gpu_cluster_folder_id">
    <rdfs:label>folder_id</rdfs:label>
    <rdfs:comment>ID of the folder that the GPU cluster belongs to.</rdfs:comment>
    <rdfs:domain rdf:resource="http://example.org/onto/class/yandex_compute_gpu_cluster"/>
    <rdfs:range rdf:resource="http://www.w3.org/2001/XMLSchema#string"/>
  </owl:DatatypeProperty>
  <owl:DatatypeProperty rdf:about="http://example.org/onto/prop/yandex_compute_gpu_cluster_gpu_cluster_id">
    <rdfs:label>gpu_cluster_id</rdfs:label>
    <rdfs:comment>ID of the GPU cluster to return.

 To get a GPU cluster ID, make a [GpuClusterService.List] request.</rdfs:comment>
    <rdfs:domain rdf:resource="http://example.org/onto/class/yandex_compute_gpu_cluster"/>
    <rdfs:range rdf:resource="http://www.w3.org/2001/XMLSchema#string"/>
  </owl:DatatypeProperty>
  <owl:DatatypeProperty rdf:about="http://example.org/onto/prop/yandex_compute_gpu_cluster_id">
    <rdfs:label>id</rdfs:label>
    <rdfs:comment>ID of the GPU cluster to return.

 To get a GPU cluster ID, make a [GpuClusterService.List] request.</rdfs:comment>
    <rdfs:domain rdf:resource="http://example.org/onto/class/yandex_compute_gpu_cluster"/>
    <rdfs:range rdf:resource="http://www.w3.org/2001/XMLSchema#string"/>
  </owl:DatatypeProperty>
  <owl:DatatypeProperty rdf:about="http://example.org/onto/prop/yandex_compute_gpu_cluster_interconnect_type">
    <rdfs:label>interconnect_type</rdfs:label>
    <rdfs:comment>Type of interconnect used for this GPU cluster.</rdfs:comment>
    <rdfs:domain rdf:resource="http://example.org/onto/class/yandex_compute_gpu_cluster"/>
    <rdfs:range rdf:resource="http://www.w3.org/2001/XMLSchema#string"/>
  </owl:DatatypeProperty>
  <owl:DatatypeProperty rdf:about="http://example.org/onto/prop/yandex_compute_gpu_cluster_labels">
    <rdfs:label>labels</rdfs:label>
    <rdfs:comment>GPU cluster labels as `key:value` pairs.</rdfs:comment>
    <rdfs:domain rdf:resource="http://example.org/onto/class/yandex_compute_gpu_cluster"/>
    <rdfs:range rdf:resource="http://www.w3.org/2001/XMLSchema#string"/>
  </owl:DatatypeProperty>
  <owl:DatatypeProperty rdf:about="http://example.org/onto/prop/yandex_compute_gpu_cluster_name">
    <rdfs:label>name</rdfs:label>
    <rdfs:comment>Name of the GPU cluster.

 The name is unique within the folder.</rdfs:comment>
    <rdfs:domain rdf:resource="http://example.org/onto/class/yandex_compute_gpu_cluster"/>
    <rdfs:range rdf:resource="http://www.w3.org/2001/XMLSchema#string"/>
  </owl:DatatypeProperty>
  <owl:DatatypeProperty rdf:about="http://example.org/onto/prop/yandex_compute_gpu_cluster_status">
    <rdfs:label>status</rdfs:label>
    <rdfs:comment>Status of the GPU cluster.</rdfs:comment>
    <rdfs:domain rdf:resource="http://example.org/onto/class/yandex_compute_gpu_cluster"/>
    <rdfs:range rdf:resource="http://www.w3.org/2001/XMLSchema#string"/>
  </owl:DatatypeProperty>
  <owl:DatatypeProperty rdf:about="http://example.org/onto/prop/yandex_compute_gpu_cluster_zone">
    <rdfs:label>zone</rdfs:label>
    <rdfs:comment>ID of the availability zone where the GPU cluster resides.</rdfs:comment>
    <rdfs:domain rdf:resource="http://example.org/onto/class/yandex_compute_gpu_cluster"/>
    <rdfs:range rdf:resource="http://www.w3.org/2001/XMLSchema#string"/>
  </owl:DatatypeProperty>
  <owl:DatatypeProperty rdf:about="http://example.org/onto/prop/yandex_compute_gpu_cluster_create">
    <rdfs:label>create</rdfs:label>
    <rdfs:comment>A string that can be [parsed as a duration](https://pkg.go.dev/time#ParseDuration) consisting of numbers and unit suffixes, such as "30s" or "2h45m". Valid time units are "s" (seconds), "m" (minutes), "h" (hours).</rdfs:comment>
    <rdfs:domain rdf:resource="http://example.org/onto/class/yandex_compute_gpu_cluster"/>
    <rdfs:range rdf:resource="http://www.w3.org/2001/XMLSchema#string"/>
  </owl:DatatypeProperty>
  <owl:DatatypeProperty rdf:about="http://example.org/onto/prop/yandex_compute_gpu_cluster_delete">
    <rdfs:label>delete</rdfs:label>
    <rdfs:comment>A string that can be [parsed as a duration](https://pkg.go.dev/time#ParseDuration) consisting of numbers and unit suffixes, such as "30s" or "2h45m". Valid time units are "s" (seconds), "m" (minutes), "h" (hours). Setting a timeout for a Delete operation is only applicable if changes are saved into state before the destroy operation occurs.</rdfs:comment>
    <rdfs:domain rdf:resource="http://example.org/onto/class/yandex_compute_gpu_cluster"/>
    <rdfs:range rdf:resource="http://www.w3.org/2001/XMLSchema#string"/>
  </owl:DatatypeProperty>
  <owl:DatatypeProperty rdf:about="http://example.org/onto/prop/yandex_compute_gpu_cluster_read">
    <rdfs:label>read</rdfs:label>
    <rdfs:comment>A string that can be [parsed as a duration](https://pkg.go.dev/time#ParseDuration) consisting of numbers and unit suffixes, such as "30s" or "2h45m". Valid time units are "s" (seconds), "m" (minutes), "h" (hours). Read operations occur during any refresh or planning operation when refresh is enabled.</rdfs:comment>
    <rdfs:domain rdf:resource="http://example.org/onto/class/yandex_compute_gpu_cluster"/>
    <rdfs:range rdf:resource="http://www.w3.org/2001/XMLSchema#string"/>
  </owl:DatatypeProperty>
  <owl:DatatypeProperty rdf:about="http://example.org/onto/prop/yandex_compute_gpu_cluster_update">
    <rdfs:label>update</rdfs:label>
    <rdfs:comment>A string that can be [parsed as a duration](https://pkg.go.dev/time#ParseDuration) consisting of numbers and unit suffixes, such as "30s" or "2h45m". Valid time units are "s" (seconds), "m" (minutes), "h" (hours).</rdfs:comment>
    <rdfs:domain rdf:resource="http://example.org/onto/class/yandex_compute_gpu_cluster"/>
    <rdfs:range rdf:resource="http://www.w3.org/2001/XMLSchema#string"/>
  </owl:DatatypeProperty>
</rdf:RDF>
