<?xml version="1.0" encoding="UTF-8"?>
<rdf:RDF
  xmlns:rdf="http://www.w3.org/1999/02/22-rdf-syntax-ns#"
  xmlns:rdfs="http://www.w3.org/2000/01/rdf-schema#"
  xmlns:owl="http://www.w3.org/2002/07/owl#"
  xmlns:xsd="http://www.w3.org/2001/XMLSchema#"
  xml:base="http://example.org/onto/">
  <owl:Class rdf:about="http://example.org/onto/class/yandex_resourcemanager_folder">
    <rdfs:label>yandex_resourcemanager_folder</rdfs:label>
    <rdfs:comment>A Folder resource. For more information, see [Folder](/docs/resource-manager/concepts/resources-hierarchy#folder).</rdfs:comment>
  </owl:Class>
  <owl:DatatypeProperty rdf:about="http://example.org/onto/prop/yandex_resourcemanager_folder_cloud_id">
    <rdfs:label>cloud_id</rdfs:label>
    <rdfs:comment>ID of the cloud that the folder belongs to.</rdfs:comment>
    <rdfs:domain rdf:resource="http://example.org/onto/class/yandex_resourcemanager_folder"/>
    <rdfs:range rdf:resource="http://www.w3.org/2001/XMLSchema#string"/>
  </owl:DatatypeProperty>
  <owl:DatatypeProperty rdf:about="http://example.org/onto/prop/yandex_resourcemanager_folder_created_at">
    <rdfs:label>created_at</rdfs:label>
    <rdfs:comment>Creation timestamp.</rdfs:comment>
    <rdfs:domain rdf:resource="http://example.org/onto/class/yandex_resourcemanager_folder"/>
    <rdfs:range rdf:resource="http://www.w3.org/2001/XMLSchema#string"/>
  </owl:DatatypeProperty>
  <owl:DatatypeProperty rdf:about="http://example.org/onto/prop/yandex_resourcemanager_folder_description">
    <rdfs:label>description</rdfs:label>
    <rdfs:comment>Description of the folder. 0-256 characters long.</rdfs:comment>
    <rdfs:domain rdf:resource="http://example.org/onto/class/yandex_resourcemanager_folder"/>
    <rdfs:range rdf:resource="http://www.w3.org/2001/XMLSchema#string"/>
  </owl:DatatypeProperty>
  <owl:DatatypeProperty rdf:about="http://example.org/onto/prop/yandex_resourcemanager_folder_folder_id">
    <rdfs:label>folder_id</rdfs:label>
    <rdfs:comment>ID of the Folder resource to return.
 To get the folder ID, use a [FolderService.List] request.</rdfs:comment>
    <rdfs:domain rdf:resource="http://example.org/onto/class/yandex_resourcemanager_folder"/>
    <rdfs:range rdf:resource="http://www.w3.org/2001/XMLSchema#string"/>
  </owl:DatatypeProperty>
  <owl:DatatypeProperty rdf:about="http://example.org/onto/prop/yandex_resourcemanager_folder_id">
    <rdfs:label>id</rdfs:label>
    <rdfs:comment>ID of the Folder resource to return.
 To get the folder ID, use a [FolderService.List] request.</rdfs:comment>
    <rdfs:domain rdf:resource="http://example.org/onto/class/yandex_resourcemanager_folder"/>
    <rdfs:range rdf:resource="http://www.w3.org/2001/XMLSchema#string"/>
  </owl:DatatypeProperty>
  <owl:DatatypeProperty rdf:about="http://example.org/onto/prop/yandex_resourcemanager_folder_labels">
    <rdfs:label>labels</rdfs:label>
    <rdfs:comment>Resource labels as `` key:value `` pairs. Maximum of 64 per resource.</rdfs:comment>
    <rdfs:domain rdf:resource="http://example.org/onto/class/yandex_resourcemanager_folder"/>
    <rdfs:range rdf:resource="http://www.w3.org/2001/XMLSchema#string"/>
  </owl:DatatypeProperty>
  <owl:DatatypeProperty rdf:about="http://example.org/onto/prop/yandex_resourcemanager_folder_name">
    <rdfs:label>name</rdfs:label>
    <rdfs:comment>Name of the folder.
 The name is unique within the cloud. 3-63 characters long.</rdfs:comment>
    <rdfs:domain rdf:resource="http://example.org/onto/class/yandex_resourcemanager_folder"/>
    <rdfs:range rdf:resource="http://www.w3.org/2001/XMLSchema#string"/>
  </owl:DatatypeProperty>
  <owl:DatatypeProperty rdf:about="http://example.org/onto/prop/yandex_resourcemanager_folder_status">
    <rdfs:label>status</rdfs:label>
    <rdfs:comment>Status of the folder.</rdfs:comment>
    <rdfs:domain rdf:resource="http://example.org/onto/class/yandex_resourcemanager_folder"/>
    <rdfs:range rdf:resource="http://www.w3.org/2001/XMLSchema#string"/>
  </owl:DatatypeProperty>
  <owl:DatatypeProperty rdf:about="http://example.org/onto/prop/yandex_resourcemanager_folder_timeouts">
    <rdfs:label>timeouts</rdfs:label>
    <rdfs:domain rdf:resource="http://example.org/onto/class/yandex_resourcemanager_folder"/>
    <rdfs:range rdf:resource="http://www.w3.org/2001/XMLSchema#string"/>
  </owl:DatatypeProperty>
</rdf:RDF>
