<?xml version="1.0" encoding="UTF-8"?>
<rdf:RDF
  xmlns:rdf="http://www.w3.org/1999/02/22-rdf-syntax-ns#"
  xmlns:rdfs="http://www.w3.org/2000/01/rdf-schema#"
  xmlns:owl="http://www.w3.org/2002/07/owl#"
  xmlns:xsd="http://www.w3.org/2001/XMLSchema#"
  xml:base="http://example.org/onto/">
  <owl:Class rdf:about="http://example.org/onto/class/yandex_mdb_greenplum_cluster">
    <rdfs:label>yandex_mdb_greenplum_cluster</rdfs:label>
    <rdfs:comment>Manages a Greenplum cluster within the Yandex Cloud. For more information, see [the official documentation](https://yandex.cloud/docs/managed-greenplum/).

Please read [Pricing for Managed Service for Greenplum](https://yandex.cloud/docs/managed-greenplum/) before using Greenplum cluster.</rdfs:comment>
  </owl:Class>
  <owl:DatatypeProperty rdf:about="http://example.org/onto/prop/yandex_mdb_greenplum_cluster_assign_public_ip">
    <rdfs:label>assign_public_ip</rdfs:label>
    <rdfs:comment>Sets whether the master hosts should get a public IP address on creation. Changing this parameter for an existing host is not supported at the moment.</rdfs:comment>
    <rdfs:domain rdf:resource="http://example.org/onto/class/yandex_mdb_greenplum_cluster"/>
    <rdfs:range rdf:resource="http://www.w3.org/2001/XMLSchema#string"/>
  </owl:DatatypeProperty>
  <owl:DatatypeProperty rdf:about="http://example.org/onto/prop/yandex_mdb_greenplum_cluster_created_at">
    <rdfs:label>created_at</rdfs:label>
    <rdfs:comment>The creation timestamp of the resource.</rdfs:comment>
    <rdfs:domain rdf:resource="http://example.org/onto/class/yandex_mdb_greenplum_cluster"/>
    <rdfs:range rdf:resource="http://www.w3.org/2001/XMLSchema#string"/>
  </owl:DatatypeProperty>
  <owl:DatatypeProperty rdf:about="http://example.org/onto/prop/yandex_mdb_greenplum_cluster_deletion_protection">
    <rdfs:label>deletion_protection</rdfs:label>
    <rdfs:comment>The `true` value means that resource is protected from accidental deletion.</rdfs:comment>
    <rdfs:domain rdf:resource="http://example.org/onto/class/yandex_mdb_greenplum_cluster"/>
    <rdfs:range rdf:resource="http://www.w3.org/2001/XMLSchema#string"/>
  </owl:DatatypeProperty>
  <owl:DatatypeProperty rdf:about="http://example.org/onto/prop/yandex_mdb_greenplum_cluster_description">
    <rdfs:label>description</rdfs:label>
    <rdfs:comment>The resource description.</rdfs:comment>
    <rdfs:domain rdf:resource="http://example.org/onto/class/yandex_mdb_greenplum_cluster"/>
    <rdfs:range rdf:resource="http://www.w3.org/2001/XMLSchema#string"/>
  </owl:DatatypeProperty>
  <owl:DatatypeProperty rdf:about="http://example.org/onto/prop/yandex_mdb_greenplum_cluster_environment">
    <rdfs:label>environment</rdfs:label>
    <rdfs:comment>Deployment environment of the Greenplum cluster. (PRODUCTION, PRESTABLE)</rdfs:comment>
    <rdfs:domain rdf:resource="http://example.org/onto/class/yandex_mdb_greenplum_cluster"/>
    <rdfs:range rdf:resource="http://www.w3.org/2001/XMLSchema#string"/>
  </owl:DatatypeProperty>
  <owl:DatatypeProperty rdf:about="http://example.org/onto/prop/yandex_mdb_greenplum_cluster_folder_id">
    <rdfs:label>folder_id</rdfs:label>
    <rdfs:comment>The folder identifier that resource belongs to. If it is not provided, the default provider `folder-id` is used.</rdfs:comment>
    <rdfs:domain rdf:resource="http://example.org/onto/class/yandex_mdb_greenplum_cluster"/>
    <rdfs:range rdf:resource="http://www.w3.org/2001/XMLSchema#string"/>
  </owl:DatatypeProperty>
  <owl:DatatypeProperty rdf:about="http://example.org/onto/prop/yandex_mdb_greenplum_cluster_greenplum_config">
    <rdfs:label>greenplum_config</rdfs:label>
    <rdfs:comment>Greenplum cluster config. Detail info in `Greenplum cluster settings` block.</rdfs:comment>
    <rdfs:domain rdf:resource="http://example.org/onto/class/yandex_mdb_greenplum_cluster"/>
    <rdfs:range rdf:resource="http://www.w3.org/2001/XMLSchema#string"/>
  </owl:DatatypeProperty>
  <owl:DatatypeProperty rdf:about="http://example.org/onto/prop/yandex_mdb_greenplum_cluster_health">
    <rdfs:label>health</rdfs:label>
    <rdfs:comment>Aggregated health of the cluster.</rdfs:comment>
    <rdfs:domain rdf:resource="http://example.org/onto/class/yandex_mdb_greenplum_cluster"/>
    <rdfs:range rdf:resource="http://www.w3.org/2001/XMLSchema#string"/>
  </owl:DatatypeProperty>
  <owl:DatatypeProperty rdf:about="http://example.org/onto/prop/yandex_mdb_greenplum_cluster_id">
    <rdfs:label>id</rdfs:label>
    <rdfs:domain rdf:resource="http://example.org/onto/class/yandex_mdb_greenplum_cluster"/>
    <rdfs:range rdf:resource="http://www.w3.org/2001/XMLSchema#string"/>
  </owl:DatatypeProperty>
  <owl:DatatypeProperty rdf:about="http://example.org/onto/prop/yandex_mdb_greenplum_cluster_labels">
    <rdfs:label>labels</rdfs:label>
    <rdfs:comment>A set of key/value label pairs which assigned to resource.</rdfs:comment>
    <rdfs:domain rdf:resource="http://example.org/onto/class/yandex_mdb_greenplum_cluster"/>
    <rdfs:range rdf:resource="http://www.w3.org/2001/XMLSchema#string"/>
  </owl:DatatypeProperty>
  <owl:DatatypeProperty rdf:about="http://example.org/onto/prop/yandex_mdb_greenplum_cluster_master_host_count">
    <rdfs:label>master_host_count</rdfs:label>
    <rdfs:comment>Number of hosts in master subcluster (1 or 2).</rdfs:comment>
    <rdfs:domain rdf:resource="http://example.org/onto/class/yandex_mdb_greenplum_cluster"/>
    <rdfs:range rdf:resource="http://www.w3.org/2001/XMLSchema#string"/>
  </owl:DatatypeProperty>
  <owl:DatatypeProperty rdf:about="http://example.org/onto/prop/yandex_mdb_greenplum_cluster_master_host_group_ids">
    <rdfs:label>master_host_group_ids</rdfs:label>
    <rdfs:comment>A list of IDs of the host groups to place master subclusters' VMs of the cluster on.</rdfs:comment>
    <rdfs:domain rdf:resource="http://example.org/onto/class/yandex_mdb_greenplum_cluster"/>
    <rdfs:range rdf:resource="http://www.w3.org/2001/XMLSchema#string"/>
  </owl:DatatypeProperty>
  <owl:DatatypeProperty rdf:about="http://example.org/onto/prop/yandex_mdb_greenplum_cluster_master_hosts">
    <rdfs:label>master_hosts</rdfs:label>
    <rdfs:comment>Info about hosts in master subcluster.</rdfs:comment>
    <rdfs:domain rdf:resource="http://example.org/onto/class/yandex_mdb_greenplum_cluster"/>
    <rdfs:range rdf:resource="http://www.w3.org/2001/XMLSchema#string"/>
  </owl:DatatypeProperty>
  <owl:DatatypeProperty rdf:about="http://example.org/onto/prop/yandex_mdb_greenplum_cluster_name">
    <rdfs:label>name</rdfs:label>
    <rdfs:comment>The resource name.</rdfs:comment>
    <rdfs:domain rdf:resource="http://example.org/onto/class/yandex_mdb_greenplum_cluster"/>
    <rdfs:range rdf:resource="http://www.w3.org/2001/XMLSchema#string"/>
  </owl:DatatypeProperty>
  <owl:DatatypeProperty rdf:about="http://example.org/onto/prop/yandex_mdb_greenplum_cluster_network_id">
    <rdfs:label>network_id</rdfs:label>
    <rdfs:comment>The `VPC Network ID` of subnets which resource attached to.</rdfs:comment>
    <rdfs:domain rdf:resource="http://example.org/onto/class/yandex_mdb_greenplum_cluster"/>
    <rdfs:range rdf:resource="http://www.w3.org/2001/XMLSchema#string"/>
  </owl:DatatypeProperty>
  <owl:DatatypeProperty rdf:about="http://example.org/onto/prop/yandex_mdb_greenplum_cluster_security_group_ids">
    <rdfs:label>security_group_ids</rdfs:label>
    <rdfs:comment>The list of security groups applied to resource or their components.</rdfs:comment>
    <rdfs:domain rdf:resource="http://example.org/onto/class/yandex_mdb_greenplum_cluster"/>
    <rdfs:range rdf:resource="http://www.w3.org/2001/XMLSchema#string"/>
  </owl:DatatypeProperty>
  <owl:DatatypeProperty rdf:about="http://example.org/onto/prop/yandex_mdb_greenplum_cluster_segment_host_count">
    <rdfs:label>segment_host_count</rdfs:label>
    <rdfs:comment>Number of hosts in segment subcluster (from 1 to 32).</rdfs:comment>
    <rdfs:domain rdf:resource="http://example.org/onto/class/yandex_mdb_greenplum_cluster"/>
    <rdfs:range rdf:resource="http://www.w3.org/2001/XMLSchema#string"/>
  </owl:DatatypeProperty>
  <owl:DatatypeProperty rdf:about="http://example.org/onto/prop/yandex_mdb_greenplum_cluster_segment_host_group_ids">
    <rdfs:label>segment_host_group_ids</rdfs:label>
    <rdfs:comment>A list of IDs of the host groups to place segment subclusters' VMs of the cluster on.</rdfs:comment>
    <rdfs:domain rdf:resource="http://example.org/onto/class/yandex_mdb_greenplum_cluster"/>
    <rdfs:range rdf:resource="http://www.w3.org/2001/XMLSchema#string"/>
  </owl:DatatypeProperty>
  <owl:DatatypeProperty rdf:about="http://example.org/onto/prop/yandex_mdb_greenplum_cluster_segment_hosts">
    <rdfs:label>segment_hosts</rdfs:label>
    <rdfs:comment>Info about hosts in segment subcluster.</rdfs:comment>
    <rdfs:domain rdf:resource="http://example.org/onto/class/yandex_mdb_greenplum_cluster"/>
    <rdfs:range rdf:resource="http://www.w3.org/2001/XMLSchema#string"/>
  </owl:DatatypeProperty>
  <owl:DatatypeProperty rdf:about="http://example.org/onto/prop/yandex_mdb_greenplum_cluster_segment_in_host">
    <rdfs:label>segment_in_host</rdfs:label>
    <rdfs:comment>Number of segments on segment host (not more then 1 + RAM/8).</rdfs:comment>
    <rdfs:domain rdf:resource="http://example.org/onto/class/yandex_mdb_greenplum_cluster"/>
    <rdfs:range rdf:resource="http://www.w3.org/2001/XMLSchema#string"/>
  </owl:DatatypeProperty>
  <owl:DatatypeProperty rdf:about="http://example.org/onto/prop/yandex_mdb_greenplum_cluster_service_account_id">
    <rdfs:label>service_account_id</rdfs:label>
    <rdfs:comment>ID of service account to use with Yandex Cloud resources (e.g. S3, Cloud Logging).</rdfs:comment>
    <rdfs:domain rdf:resource="http://example.org/onto/class/yandex_mdb_greenplum_cluster"/>
    <rdfs:range rdf:resource="http://www.w3.org/2001/XMLSchema#string"/>
  </owl:DatatypeProperty>
  <owl:DatatypeProperty rdf:about="http://example.org/onto/prop/yandex_mdb_greenplum_cluster_status">
    <rdfs:label>status</rdfs:label>
    <rdfs:comment>Status of the cluster.</rdfs:comment>
    <rdfs:domain rdf:resource="http://example.org/onto/class/yandex_mdb_greenplum_cluster"/>
    <rdfs:range rdf:resource="http://www.w3.org/2001/XMLSchema#string"/>
  </owl:DatatypeProperty>
  <owl:DatatypeProperty rdf:about="http://example.org/onto/prop/yandex_mdb_greenplum_cluster_subnet_id">
    <rdfs:label>subnet_id</rdfs:label>
    <rdfs:comment>The ID of the subnet, to which the hosts belongs. The subnet must be a part of the network to which the cluster belongs.</rdfs:comment>
    <rdfs:domain rdf:resource="http://example.org/onto/class/yandex_mdb_greenplum_cluster"/>
    <rdfs:range rdf:resource="http://www.w3.org/2001/XMLSchema#string"/>
  </owl:DatatypeProperty>
  <owl:DatatypeProperty rdf:about="http://example.org/onto/prop/yandex_mdb_greenplum_cluster_user_name">
    <rdfs:label>user_name</rdfs:label>
    <rdfs:comment>Greenplum cluster admin user name.</rdfs:comment>
    <rdfs:domain rdf:resource="http://example.org/onto/class/yandex_mdb_greenplum_cluster"/>
    <rdfs:range rdf:resource="http://www.w3.org/2001/XMLSchema#string"/>
  </owl:DatatypeProperty>
  <owl:DatatypeProperty rdf:about="http://example.org/onto/prop/yandex_mdb_greenplum_cluster_user_password">
    <rdfs:label>user_password</rdfs:label>
    <rdfs:comment>Greenplum cluster admin password name.</rdfs:comment>
    <rdfs:domain rdf:resource="http://example.org/onto/class/yandex_mdb_greenplum_cluster"/>
    <rdfs:range rdf:resource="http://www.w3.org/2001/XMLSchema#string"/>
  </owl:DatatypeProperty>
  <owl:DatatypeProperty rdf:about="http://example.org/onto/prop/yandex_mdb_greenplum_cluster_version">
    <rdfs:label>version</rdfs:label>
    <rdfs:comment>Version of the Greenplum cluster. (`6.28`)</rdfs:comment>
    <rdfs:domain rdf:resource="http://example.org/onto/class/yandex_mdb_greenplum_cluster"/>
    <rdfs:range rdf:resource="http://www.w3.org/2001/XMLSchema#string"/>
  </owl:DatatypeProperty>
  <owl:DatatypeProperty rdf:about="http://example.org/onto/prop/yandex_mdb_greenplum_cluster_zone">
    <rdfs:label>zone</rdfs:label>
    <rdfs:comment>The [availability zone](https://yandex.cloud/docs/overview/concepts/geo-scope) where resource is located. If it is not provided, the default provider zone will be used.</rdfs:comment>
    <rdfs:domain rdf:resource="http://example.org/onto/class/yandex_mdb_greenplum_cluster"/>
    <rdfs:range rdf:resource="http://www.w3.org/2001/XMLSchema#string"/>
  </owl:DatatypeProperty>
  <owl:DatatypeProperty rdf:about="http://example.org/onto/prop/yandex_mdb_greenplum_cluster_data_lens">
    <rdfs:label>data_lens</rdfs:label>
    <rdfs:comment>Allow access for [Yandex DataLens](https://yandex.cloud/services/datalens).</rdfs:comment>
    <rdfs:domain rdf:resource="http://example.org/onto/class/yandex_mdb_greenplum_cluster"/>
    <rdfs:range rdf:resource="http://www.w3.org/2001/XMLSchema#string"/>
  </owl:DatatypeProperty>
  <owl:DatatypeProperty rdf:about="http://example.org/onto/prop/yandex_mdb_greenplum_cluster_data_transfer">
    <rdfs:label>data_transfer</rdfs:label>
    <rdfs:comment>Allow access for [DataTransfer](https://yandex.cloud/services/data-transfer)</rdfs:comment>
    <rdfs:domain rdf:resource="http://example.org/onto/class/yandex_mdb_greenplum_cluster"/>
    <rdfs:range rdf:resource="http://www.w3.org/2001/XMLSchema#string"/>
  </owl:DatatypeProperty>
  <owl:DatatypeProperty rdf:about="http://example.org/onto/prop/yandex_mdb_greenplum_cluster_web_sql">
    <rdfs:label>web_sql</rdfs:label>
    <rdfs:comment>Allows access for [SQL queries in the management console](https://yandex.cloud/docs/managed-mysql/operations/web-sql-query).</rdfs:comment>
    <rdfs:domain rdf:resource="http://example.org/onto/class/yandex_mdb_greenplum_cluster"/>
    <rdfs:range rdf:resource="http://www.w3.org/2001/XMLSchema#string"/>
  </owl:DatatypeProperty>
  <owl:DatatypeProperty rdf:about="http://example.org/onto/prop/yandex_mdb_greenplum_cluster_yandex_query">
    <rdfs:label>yandex_query</rdfs:label>
    <rdfs:comment>Allow access for [Yandex Query](https://yandex.cloud/services/query)</rdfs:comment>
    <rdfs:domain rdf:resource="http://example.org/onto/class/yandex_mdb_greenplum_cluster"/>
    <rdfs:range rdf:resource="http://www.w3.org/2001/XMLSchema#string"/>
  </owl:DatatypeProperty>
  <owl:DatatypeProperty rdf:about="http://example.org/onto/prop/yandex_mdb_greenplum_cluster_analyze_timeout">
    <rdfs:label>analyze_timeout</rdfs:label>
    <rdfs:comment>Maximum duration of the `ANALYZE` operation, in seconds. The default value is `36000`. As soon as this period expires, the `ANALYZE` operation will be forced to terminate.</rdfs:comment>
    <rdfs:domain rdf:resource="http://example.org/onto/class/yandex_mdb_greenplum_cluster"/>
    <rdfs:range rdf:resource="http://www.w3.org/2001/XMLSchema#string"/>
  </owl:DatatypeProperty>
  <owl:DatatypeProperty rdf:about="http://example.org/onto/prop/yandex_mdb_greenplum_cluster_start_time">
    <rdfs:label>start_time</rdfs:label>
    <rdfs:comment>Time of day in 'HH:MM' format when scripts should run.</rdfs:comment>
    <rdfs:domain rdf:resource="http://example.org/onto/class/yandex_mdb_greenplum_cluster"/>
    <rdfs:range rdf:resource="http://www.w3.org/2001/XMLSchema#string"/>
  </owl:DatatypeProperty>
  <owl:DatatypeProperty rdf:about="http://example.org/onto/prop/yandex_mdb_greenplum_cluster_vacuum_timeout">
    <rdfs:label>vacuum_timeout</rdfs:label>
    <rdfs:comment>Maximum duration of the `VACUUM` operation, in seconds. The default value is `36000`. As soon as this period expires, the `VACUUM` operation will be forced to terminate.</rdfs:comment>
    <rdfs:domain rdf:resource="http://example.org/onto/class/yandex_mdb_greenplum_cluster"/>
    <rdfs:range rdf:resource="http://www.w3.org/2001/XMLSchema#string"/>
  </owl:DatatypeProperty>
  <owl:DatatypeProperty rdf:about="http://example.org/onto/prop/yandex_mdb_greenplum_cluster_enable">
    <rdfs:label>enable</rdfs:label>
    <rdfs:comment>Flag that indicates whether script is enabled.</rdfs:comment>
    <rdfs:domain rdf:resource="http://example.org/onto/class/yandex_mdb_greenplum_cluster"/>
    <rdfs:range rdf:resource="http://www.w3.org/2001/XMLSchema#string"/>
  </owl:DatatypeProperty>
  <owl:DatatypeProperty rdf:about="http://example.org/onto/prop/yandex_mdb_greenplum_cluster_ignore_users">
    <rdfs:label>ignore_users</rdfs:label>
    <rdfs:comment>List of users to ignore when considering queries to terminate.</rdfs:comment>
    <rdfs:domain rdf:resource="http://example.org/onto/class/yandex_mdb_greenplum_cluster"/>
    <rdfs:range rdf:resource="http://www.w3.org/2001/XMLSchema#string"/>
  </owl:DatatypeProperty>
  <owl:DatatypeProperty rdf:about="http://example.org/onto/prop/yandex_mdb_greenplum_cluster_max_age">
    <rdfs:label>max_age</rdfs:label>
    <rdfs:comment>Maximum duration for this type of queries (in seconds).</rdfs:comment>
    <rdfs:domain rdf:resource="http://example.org/onto/class/yandex_mdb_greenplum_cluster"/>
    <rdfs:range rdf:resource="http://www.w3.org/2001/XMLSchema#string"/>
  </owl:DatatypeProperty>
  <owl:DatatypeProperty rdf:about="http://example.org/onto/prop/yandex_mdb_greenplum_cluster_enable">
    <rdfs:label>enable</rdfs:label>
    <rdfs:comment>Flag that indicates whether script is enabled.</rdfs:comment>
    <rdfs:domain rdf:resource="http://example.org/onto/class/yandex_mdb_greenplum_cluster"/>
    <rdfs:range rdf:resource="http://www.w3.org/2001/XMLSchema#string"/>
  </owl:DatatypeProperty>
  <owl:DatatypeProperty rdf:about="http://example.org/onto/prop/yandex_mdb_greenplum_cluster_ignore_users">
    <rdfs:label>ignore_users</rdfs:label>
    <rdfs:comment>List of users to ignore when considering queries to terminate.</rdfs:comment>
    <rdfs:domain rdf:resource="http://example.org/onto/class/yandex_mdb_greenplum_cluster"/>
    <rdfs:range rdf:resource="http://www.w3.org/2001/XMLSchema#string"/>
  </owl:DatatypeProperty>
  <owl:DatatypeProperty rdf:about="http://example.org/onto/prop/yandex_mdb_greenplum_cluster_max_age">
    <rdfs:label>max_age</rdfs:label>
    <rdfs:comment>Maximum duration for this type of queries (in seconds).</rdfs:comment>
    <rdfs:domain rdf:resource="http://example.org/onto/class/yandex_mdb_greenplum_cluster"/>
    <rdfs:range rdf:resource="http://www.w3.org/2001/XMLSchema#string"/>
  </owl:DatatypeProperty>
  <owl:DatatypeProperty rdf:about="http://example.org/onto/prop/yandex_mdb_greenplum_cluster_enable">
    <rdfs:label>enable</rdfs:label>
    <rdfs:comment>Flag that indicates whether script is enabled.</rdfs:comment>
    <rdfs:domain rdf:resource="http://example.org/onto/class/yandex_mdb_greenplum_cluster"/>
    <rdfs:range rdf:resource="http://www.w3.org/2001/XMLSchema#string"/>
  </owl:DatatypeProperty>
  <owl:DatatypeProperty rdf:about="http://example.org/onto/prop/yandex_mdb_greenplum_cluster_ignore_users">
    <rdfs:label>ignore_users</rdfs:label>
    <rdfs:comment>List of users to ignore when considering queries to terminate.</rdfs:comment>
    <rdfs:domain rdf:resource="http://example.org/onto/class/yandex_mdb_greenplum_cluster"/>
    <rdfs:range rdf:resource="http://www.w3.org/2001/XMLSchema#string"/>
  </owl:DatatypeProperty>
  <owl:DatatypeProperty rdf:about="http://example.org/onto/prop/yandex_mdb_greenplum_cluster_max_age">
    <rdfs:label>max_age</rdfs:label>
    <rdfs:comment>Maximum duration for this type of queries (in seconds).</rdfs:comment>
    <rdfs:domain rdf:resource="http://example.org/onto/class/yandex_mdb_greenplum_cluster"/>
    <rdfs:range rdf:resource="http://www.w3.org/2001/XMLSchema#string"/>
  </owl:DatatypeProperty>
  <owl:DatatypeProperty rdf:about="http://example.org/onto/prop/yandex_mdb_greenplum_cluster_hours">
    <rdfs:label>hours</rdfs:label>
    <rdfs:comment>The hour at which backup will be started (UTC).</rdfs:comment>
    <rdfs:domain rdf:resource="http://example.org/onto/class/yandex_mdb_greenplum_cluster"/>
    <rdfs:range rdf:resource="http://www.w3.org/2001/XMLSchema#string"/>
  </owl:DatatypeProperty>
  <owl:DatatypeProperty rdf:about="http://example.org/onto/prop/yandex_mdb_greenplum_cluster_minutes">
    <rdfs:label>minutes</rdfs:label>
    <rdfs:comment>The minute at which backup will be started (UTC).</rdfs:comment>
    <rdfs:domain rdf:resource="http://example.org/onto/class/yandex_mdb_greenplum_cluster"/>
    <rdfs:range rdf:resource="http://www.w3.org/2001/XMLSchema#string"/>
  </owl:DatatypeProperty>
  <owl:DatatypeProperty rdf:about="http://example.org/onto/prop/yandex_mdb_greenplum_cluster_enable">
    <rdfs:label>enable</rdfs:label>
    <rdfs:comment>Whether to use cloud storage or not.</rdfs:comment>
    <rdfs:domain rdf:resource="http://example.org/onto/class/yandex_mdb_greenplum_cluster"/>
    <rdfs:range rdf:resource="http://www.w3.org/2001/XMLSchema#string"/>
  </owl:DatatypeProperty>
  <owl:DatatypeProperty rdf:about="http://example.org/onto/prop/yandex_mdb_greenplum_cluster_command_center_enabled">
    <rdfs:label>command_center_enabled</rdfs:label>
    <rdfs:comment>Deliver Yandex Command Center's logs to Cloud Logging.</rdfs:comment>
    <rdfs:domain rdf:resource="http://example.org/onto/class/yandex_mdb_greenplum_cluster"/>
    <rdfs:range rdf:resource="http://www.w3.org/2001/XMLSchema#string"/>
  </owl:DatatypeProperty>
  <owl:DatatypeProperty rdf:about="http://example.org/onto/prop/yandex_mdb_greenplum_cluster_enabled">
    <rdfs:label>enabled</rdfs:label>
    <rdfs:comment>Flag that indicates whether log delivery to Cloud Logging is enabled.</rdfs:comment>
    <rdfs:domain rdf:resource="http://example.org/onto/class/yandex_mdb_greenplum_cluster"/>
    <rdfs:range rdf:resource="http://www.w3.org/2001/XMLSchema#string"/>
  </owl:DatatypeProperty>
  <owl:DatatypeProperty rdf:about="http://example.org/onto/prop/yandex_mdb_greenplum_cluster_folder_id">
    <rdfs:label>folder_id</rdfs:label>
    <rdfs:comment>ID of folder to which deliver logs.</rdfs:comment>
    <rdfs:domain rdf:resource="http://example.org/onto/class/yandex_mdb_greenplum_cluster"/>
    <rdfs:range rdf:resource="http://www.w3.org/2001/XMLSchema#string"/>
  </owl:DatatypeProperty>
  <owl:DatatypeProperty rdf:about="http://example.org/onto/prop/yandex_mdb_greenplum_cluster_greenplum_enabled">
    <rdfs:label>greenplum_enabled</rdfs:label>
    <rdfs:comment>Deliver Greenplum's logs to Cloud Logging.</rdfs:comment>
    <rdfs:domain rdf:resource="http://example.org/onto/class/yandex_mdb_greenplum_cluster"/>
    <rdfs:range rdf:resource="http://www.w3.org/2001/XMLSchema#string"/>
  </owl:DatatypeProperty>
  <owl:DatatypeProperty rdf:about="http://example.org/onto/prop/yandex_mdb_greenplum_cluster_log_group_id">
    <rdfs:label>log_group_id</rdfs:label>
    <rdfs:comment>Cloud Logging group ID to send logs to.</rdfs:comment>
    <rdfs:domain rdf:resource="http://example.org/onto/class/yandex_mdb_greenplum_cluster"/>
    <rdfs:range rdf:resource="http://www.w3.org/2001/XMLSchema#string"/>
  </owl:DatatypeProperty>
  <owl:DatatypeProperty rdf:about="http://example.org/onto/prop/yandex_mdb_greenplum_cluster_pooler_enabled">
    <rdfs:label>pooler_enabled</rdfs:label>
    <rdfs:comment>Deliver connection pooler's logs to Cloud Logging.</rdfs:comment>
    <rdfs:domain rdf:resource="http://example.org/onto/class/yandex_mdb_greenplum_cluster"/>
    <rdfs:range rdf:resource="http://www.w3.org/2001/XMLSchema#string"/>
  </owl:DatatypeProperty>
  <owl:DatatypeProperty rdf:about="http://example.org/onto/prop/yandex_mdb_greenplum_cluster_day">
    <rdfs:label>day</rdfs:label>
    <rdfs:comment>Day of the week (in `DDD` format). Allowed values: `MON`, `TUE`, `WED`, `THU`, `FRI`, `SAT`, `SUN`.</rdfs:comment>
    <rdfs:domain rdf:resource="http://example.org/onto/class/yandex_mdb_greenplum_cluster"/>
    <rdfs:range rdf:resource="http://www.w3.org/2001/XMLSchema#string"/>
  </owl:DatatypeProperty>
  <owl:DatatypeProperty rdf:about="http://example.org/onto/prop/yandex_mdb_greenplum_cluster_hour">
    <rdfs:label>hour</rdfs:label>
    <rdfs:comment>Hour of the day in UTC (in `HH` format). Allowed value is between 0 and 23.</rdfs:comment>
    <rdfs:domain rdf:resource="http://example.org/onto/class/yandex_mdb_greenplum_cluster"/>
    <rdfs:range rdf:resource="http://www.w3.org/2001/XMLSchema#string"/>
  </owl:DatatypeProperty>
  <owl:DatatypeProperty rdf:about="http://example.org/onto/prop/yandex_mdb_greenplum_cluster_type">
    <rdfs:label>type</rdfs:label>
    <rdfs:comment>Type of maintenance window. Can be either `ANYTIME` or `WEEKLY`. A day and hour of window need to be specified with weekly window.</rdfs:comment>
    <rdfs:domain rdf:resource="http://example.org/onto/class/yandex_mdb_greenplum_cluster"/>
    <rdfs:range rdf:resource="http://www.w3.org/2001/XMLSchema#string"/>
  </owl:DatatypeProperty>
  <owl:DatatypeProperty rdf:about="http://example.org/onto/prop/yandex_mdb_greenplum_cluster_disk_size">
    <rdfs:label>disk_size</rdfs:label>
    <rdfs:comment>Volume of the storage available to a host, in gigabytes.</rdfs:comment>
    <rdfs:domain rdf:resource="http://example.org/onto/class/yandex_mdb_greenplum_cluster"/>
    <rdfs:range rdf:resource="http://www.w3.org/2001/XMLSchema#string"/>
  </owl:DatatypeProperty>
  <owl:DatatypeProperty rdf:about="http://example.org/onto/prop/yandex_mdb_greenplum_cluster_disk_type_id">
    <rdfs:label>disk_type_id</rdfs:label>
    <rdfs:comment>Type of the storage of Greenplum hosts - environment default is used if missing.</rdfs:comment>
    <rdfs:domain rdf:resource="http://example.org/onto/class/yandex_mdb_greenplum_cluster"/>
    <rdfs:range rdf:resource="http://www.w3.org/2001/XMLSchema#string"/>
  </owl:DatatypeProperty>
  <owl:DatatypeProperty rdf:about="http://example.org/onto/prop/yandex_mdb_greenplum_cluster_resource_preset_id">
    <rdfs:label>resource_preset_id</rdfs:label>
    <rdfs:comment>The ID of the preset for computational resources available to a host (CPU, memory etc.). For more information, see [the official documentation](https://yandex.cloud/ru/docs/managed-greenplum/concepts/instance-types).</rdfs:comment>
    <rdfs:domain rdf:resource="http://example.org/onto/class/yandex_mdb_greenplum_cluster"/>
    <rdfs:range rdf:resource="http://www.w3.org/2001/XMLSchema#string"/>
  </owl:DatatypeProperty>
  <owl:DatatypeProperty rdf:about="http://example.org/onto/prop/yandex_mdb_greenplum_cluster_pool_client_idle_timeout">
    <rdfs:label>pool_client_idle_timeout</rdfs:label>
    <rdfs:comment>Value for `pool_client_idle_timeout` [parameter in Odyssey](https://github.com/yandex/odyssey/blob/master/documentation/configuration.md#pool_ttl-integer).</rdfs:comment>
    <rdfs:domain rdf:resource="http://example.org/onto/class/yandex_mdb_greenplum_cluster"/>
    <rdfs:range rdf:resource="http://www.w3.org/2001/XMLSchema#string"/>
  </owl:DatatypeProperty>
  <owl:DatatypeProperty rdf:about="http://example.org/onto/prop/yandex_mdb_greenplum_cluster_pool_size">
    <rdfs:label>pool_size</rdfs:label>
    <rdfs:comment>Value for `pool_size` [parameter in Odyssey](https://github.com/yandex/odyssey/blob/master/documentation/configuration.md#pool_size-integer).</rdfs:comment>
    <rdfs:domain rdf:resource="http://example.org/onto/class/yandex_mdb_greenplum_cluster"/>
    <rdfs:range rdf:resource="http://www.w3.org/2001/XMLSchema#string"/>
  </owl:DatatypeProperty>
  <owl:DatatypeProperty rdf:about="http://example.org/onto/prop/yandex_mdb_greenplum_cluster_pooling_mode">
    <rdfs:label>pooling_mode</rdfs:label>
    <rdfs:comment>Mode that the connection pooler is working in. See descriptions of all modes in the [documentation for Odyssey](https://github.com/yandex/odyssey/blob/master/documentation/configuration.md#pool-string.</rdfs:comment>
    <rdfs:domain rdf:resource="http://example.org/onto/class/yandex_mdb_greenplum_cluster"/>
    <rdfs:range rdf:resource="http://www.w3.org/2001/XMLSchema#string"/>
  </owl:DatatypeProperty>
  <owl:DatatypeProperty rdf:about="http://example.org/onto/prop/yandex_mdb_greenplum_cluster_connection_timeout">
    <rdfs:label>connection_timeout</rdfs:label>
    <rdfs:comment>The Tomcat server connection timeout for read operations in seconds. Value is between 5 and 600.</rdfs:comment>
    <rdfs:domain rdf:resource="http://example.org/onto/class/yandex_mdb_greenplum_cluster"/>
    <rdfs:range rdf:resource="http://www.w3.org/2001/XMLSchema#string"/>
  </owl:DatatypeProperty>
  <owl:DatatypeProperty rdf:about="http://example.org/onto/prop/yandex_mdb_greenplum_cluster_max_threads">
    <rdfs:label>max_threads</rdfs:label>
    <rdfs:comment>The maximum number of PXF tomcat threads. Value is between 1 and 1024.</rdfs:comment>
    <rdfs:domain rdf:resource="http://example.org/onto/class/yandex_mdb_greenplum_cluster"/>
    <rdfs:range rdf:resource="http://www.w3.org/2001/XMLSchema#string"/>
  </owl:DatatypeProperty>
  <owl:DatatypeProperty rdf:about="http://example.org/onto/prop/yandex_mdb_greenplum_cluster_pool_allow_core_thread_timeout">
    <rdfs:label>pool_allow_core_thread_timeout</rdfs:label>
    <rdfs:comment>Identifies whether or not core streaming threads are allowed to time out.</rdfs:comment>
    <rdfs:domain rdf:resource="http://example.org/onto/class/yandex_mdb_greenplum_cluster"/>
    <rdfs:range rdf:resource="http://www.w3.org/2001/XMLSchema#string"/>
  </owl:DatatypeProperty>
  <owl:DatatypeProperty rdf:about="http://example.org/onto/prop/yandex_mdb_greenplum_cluster_pool_core_size">
    <rdfs:label>pool_core_size</rdfs:label>
    <rdfs:comment>The number of core streaming threads. Value is between 1 and 1024.</rdfs:comment>
    <rdfs:domain rdf:resource="http://example.org/onto/class/yandex_mdb_greenplum_cluster"/>
    <rdfs:range rdf:resource="http://www.w3.org/2001/XMLSchema#string"/>
  </owl:DatatypeProperty>
  <owl:DatatypeProperty rdf:about="http://example.org/onto/prop/yandex_mdb_greenplum_cluster_pool_max_size">
    <rdfs:label>pool_max_size</rdfs:label>
    <rdfs:comment>The maximum allowed number of core streaming threads. Value is between 1 and 1024.</rdfs:comment>
    <rdfs:domain rdf:resource="http://example.org/onto/class/yandex_mdb_greenplum_cluster"/>
    <rdfs:range rdf:resource="http://www.w3.org/2001/XMLSchema#string"/>
  </owl:DatatypeProperty>
  <owl:DatatypeProperty rdf:about="http://example.org/onto/prop/yandex_mdb_greenplum_cluster_pool_queue_capacity">
    <rdfs:label>pool_queue_capacity</rdfs:label>
    <rdfs:comment>The capacity of the core streaming thread pool queue. Value is positive.</rdfs:comment>
    <rdfs:domain rdf:resource="http://example.org/onto/class/yandex_mdb_greenplum_cluster"/>
    <rdfs:range rdf:resource="http://www.w3.org/2001/XMLSchema#string"/>
  </owl:DatatypeProperty>
  <owl:DatatypeProperty rdf:about="http://example.org/onto/prop/yandex_mdb_greenplum_cluster_upload_timeout">
    <rdfs:label>upload_timeout</rdfs:label>
    <rdfs:comment>The Tomcat server connection timeout for write operations in seconds. Value is between 5 and 600.</rdfs:comment>
    <rdfs:domain rdf:resource="http://example.org/onto/class/yandex_mdb_greenplum_cluster"/>
    <rdfs:range rdf:resource="http://www.w3.org/2001/XMLSchema#string"/>
  </owl:DatatypeProperty>
  <owl:DatatypeProperty rdf:about="http://example.org/onto/prop/yandex_mdb_greenplum_cluster_xms">
    <rdfs:label>xms</rdfs:label>
    <rdfs:comment>Maximum JVM heap size for PXF daemon. Value is between 64 and 16384.</rdfs:comment>
    <rdfs:domain rdf:resource="http://example.org/onto/class/yandex_mdb_greenplum_cluster"/>
    <rdfs:range rdf:resource="http://www.w3.org/2001/XMLSchema#string"/>
  </owl:DatatypeProperty>
  <owl:DatatypeProperty rdf:about="http://example.org/onto/prop/yandex_mdb_greenplum_cluster_xmx">
    <rdfs:label>xmx</rdfs:label>
    <rdfs:comment>Initial JVM heap size for PXF daemon. Value is between 64 and 16384.</rdfs:comment>
    <rdfs:domain rdf:resource="http://example.org/onto/class/yandex_mdb_greenplum_cluster"/>
    <rdfs:range rdf:resource="http://www.w3.org/2001/XMLSchema#string"/>
  </owl:DatatypeProperty>
  <owl:DatatypeProperty rdf:about="http://example.org/onto/prop/yandex_mdb_greenplum_cluster_disk_size">
    <rdfs:label>disk_size</rdfs:label>
    <rdfs:comment>Volume of the storage available to a host, in gigabytes.</rdfs:comment>
    <rdfs:domain rdf:resource="http://example.org/onto/class/yandex_mdb_greenplum_cluster"/>
    <rdfs:range rdf:resource="http://www.w3.org/2001/XMLSchema#string"/>
  </owl:DatatypeProperty>
  <owl:DatatypeProperty rdf:about="http://example.org/onto/prop/yandex_mdb_greenplum_cluster_disk_type_id">
    <rdfs:label>disk_type_id</rdfs:label>
    <rdfs:comment>Type of the storage of Greenplum hosts - environment default is used if missing.</rdfs:comment>
    <rdfs:domain rdf:resource="http://example.org/onto/class/yandex_mdb_greenplum_cluster"/>
    <rdfs:range rdf:resource="http://www.w3.org/2001/XMLSchema#string"/>
  </owl:DatatypeProperty>
  <owl:DatatypeProperty rdf:about="http://example.org/onto/prop/yandex_mdb_greenplum_cluster_resource_preset_id">
    <rdfs:label>resource_preset_id</rdfs:label>
    <rdfs:comment>The ID of the preset for computational resources available to a host (CPU, memory etc.). For more information, see [the official documentation](https://yandex.cloud/ru/docs/managed-greenplum/concepts/instance-types).</rdfs:comment>
    <rdfs:domain rdf:resource="http://example.org/onto/class/yandex_mdb_greenplum_cluster"/>
    <rdfs:range rdf:resource="http://www.w3.org/2001/XMLSchema#string"/>
  </owl:DatatypeProperty>
  <owl:DatatypeProperty rdf:about="http://example.org/onto/prop/yandex_mdb_greenplum_cluster_create">
    <rdfs:label>create</rdfs:label>
    <rdfs:domain rdf:resource="http://example.org/onto/class/yandex_mdb_greenplum_cluster"/>
    <rdfs:range rdf:resource="http://www.w3.org/2001/XMLSchema#string"/>
  </owl:DatatypeProperty>
  <owl:DatatypeProperty rdf:about="http://example.org/onto/prop/yandex_mdb_greenplum_cluster_delete">
    <rdfs:label>delete</rdfs:label>
    <rdfs:domain rdf:resource="http://example.org/onto/class/yandex_mdb_greenplum_cluster"/>
    <rdfs:range rdf:resource="http://www.w3.org/2001/XMLSchema#string"/>
  </owl:DatatypeProperty>
  <owl:DatatypeProperty rdf:about="http://example.org/onto/prop/yandex_mdb_greenplum_cluster_update">
    <rdfs:label>update</rdfs:label>
    <rdfs:domain rdf:resource="http://example.org/onto/class/yandex_mdb_greenplum_cluster"/>
    <rdfs:range rdf:resource="http://www.w3.org/2001/XMLSchema#string"/>
  </owl:DatatypeProperty>
</rdf:RDF>
