<?xml version="1.0" encoding="UTF-8"?>
<rdf:RDF
  xmlns:rdf="http://www.w3.org/1999/02/22-rdf-syntax-ns#"
  xmlns:rdfs="http://www.w3.org/2000/01/rdf-schema#"
  xmlns:owl="http://www.w3.org/2002/07/owl#"
  xmlns:xsd="http://www.w3.org/2001/XMLSchema#"
  xml:base="http://example.org/onto/">
  <owl:Class rdf:about="http://example.org/onto/class/yandex_storage_object">
    <rdfs:label>yandex_storage_object</rdfs:label>
    <rdfs:comment>Allows management of [Yandex Cloud Storage Object](https://yandex.cloud/docs/storage/concepts/object).</rdfs:comment>
  </owl:Class>
  <owl:DatatypeProperty rdf:about="http://example.org/onto/prop/yandex_storage_object_access_key">
    <rdfs:label>access_key</rdfs:label>
    <rdfs:comment>The access key to use when applying changes. This value can also be provided as `storage_access_key` specified in provider config (explicitly or within `shared_credentials_file`) is used.</rdfs:comment>
    <rdfs:domain rdf:resource="http://example.org/onto/class/yandex_storage_object"/>
    <rdfs:range rdf:resource="http://www.w3.org/2001/XMLSchema#string"/>
  </owl:DatatypeProperty>
  <owl:DatatypeProperty rdf:about="http://example.org/onto/prop/yandex_storage_object_acl">
    <rdfs:label>acl</rdfs:label>
    <rdfs:comment>The [predefined ACL](https://yandex.cloud/docs/storage/concepts/acl#predefined_acls) to apply. Defaults to `private`.

~> To change ACL after creation, the service account to which used access and secret keys correspond should have `storage.admin` role, though this role is not necessary to be able to create an object with any ACL.</rdfs:comment>
    <rdfs:domain rdf:resource="http://example.org/onto/class/yandex_storage_object"/>
    <rdfs:range rdf:resource="http://www.w3.org/2001/XMLSchema#string"/>
  </owl:DatatypeProperty>
  <owl:DatatypeProperty rdf:about="http://example.org/onto/prop/yandex_storage_object_bucket">
    <rdfs:label>bucket</rdfs:label>
    <rdfs:comment>The name of the containing bucket.</rdfs:comment>
    <rdfs:domain rdf:resource="http://example.org/onto/class/yandex_storage_object"/>
    <rdfs:range rdf:resource="http://www.w3.org/2001/XMLSchema#string"/>
  </owl:DatatypeProperty>
  <owl:DatatypeProperty rdf:about="http://example.org/onto/prop/yandex_storage_object_content">
    <rdfs:label>content</rdfs:label>
    <rdfs:comment>Literal string value to use as the object content, which will be uploaded as UTF-8-encoded text. Conflicts with `source` and `content_base64`.</rdfs:comment>
    <rdfs:domain rdf:resource="http://example.org/onto/class/yandex_storage_object"/>
    <rdfs:range rdf:resource="http://www.w3.org/2001/XMLSchema#string"/>
  </owl:DatatypeProperty>
  <owl:DatatypeProperty rdf:about="http://example.org/onto/prop/yandex_storage_object_content_base64">
    <rdfs:label>content_base64</rdfs:label>
    <rdfs:comment>Base64-encoded data that will be decoded and uploaded as raw bytes for the object content. This allows safely uploading non-UTF8 binary data, but is recommended only for small content such as the result of the `gzipbase64` function with small text strings. For larger objects, use `source` to stream the content from a disk file. Conflicts with `source` and `content`.</rdfs:comment>
    <rdfs:domain rdf:resource="http://example.org/onto/class/yandex_storage_object"/>
    <rdfs:range rdf:resource="http://www.w3.org/2001/XMLSchema#string"/>
  </owl:DatatypeProperty>
  <owl:DatatypeProperty rdf:about="http://example.org/onto/prop/yandex_storage_object_content_type">
    <rdfs:label>content_type</rdfs:label>
    <rdfs:comment>A standard MIME type describing the format of the object data, e.g. `application/octet-stream`. All Valid MIME Types are valid for this input.</rdfs:comment>
    <rdfs:domain rdf:resource="http://example.org/onto/class/yandex_storage_object"/>
    <rdfs:range rdf:resource="http://www.w3.org/2001/XMLSchema#string"/>
  </owl:DatatypeProperty>
  <owl:DatatypeProperty rdf:about="http://example.org/onto/prop/yandex_storage_object_id">
    <rdfs:label>id</rdfs:label>
    <rdfs:domain rdf:resource="http://example.org/onto/class/yandex_storage_object"/>
    <rdfs:range rdf:resource="http://www.w3.org/2001/XMLSchema#string"/>
  </owl:DatatypeProperty>
  <owl:DatatypeProperty rdf:about="http://example.org/onto/prop/yandex_storage_object_key">
    <rdfs:label>key</rdfs:label>
    <rdfs:comment>The name of the object once it is in the bucket.</rdfs:comment>
    <rdfs:domain rdf:resource="http://example.org/onto/class/yandex_storage_object"/>
    <rdfs:range rdf:resource="http://www.w3.org/2001/XMLSchema#string"/>
  </owl:DatatypeProperty>
  <owl:DatatypeProperty rdf:about="http://example.org/onto/prop/yandex_storage_object_object_lock_legal_hold_status">
    <rdfs:label>object_lock_legal_hold_status</rdfs:label>
    <rdfs:comment>Specifies a [legal hold status](https://yandex.cloud/docs/storage/concepts/object-lock#types) of an object. Requires `object_lock_configuration` to be enabled on a bucket.</rdfs:comment>
    <rdfs:domain rdf:resource="http://example.org/onto/class/yandex_storage_object"/>
    <rdfs:range rdf:resource="http://www.w3.org/2001/XMLSchema#string"/>
  </owl:DatatypeProperty>
  <owl:DatatypeProperty rdf:about="http://example.org/onto/prop/yandex_storage_object_object_lock_mode">
    <rdfs:label>object_lock_mode</rdfs:label>
    <rdfs:comment>Specifies a type of object lock. One of `["GOVERNANCE", "COMPLIANCE"]`. It must be set simultaneously with `object_lock_retain_until_date`. Requires `object_lock_configuration` to be enabled on a bucket.</rdfs:comment>
    <rdfs:domain rdf:resource="http://example.org/onto/class/yandex_storage_object"/>
    <rdfs:range rdf:resource="http://www.w3.org/2001/XMLSchema#string"/>
  </owl:DatatypeProperty>
  <owl:DatatypeProperty rdf:about="http://example.org/onto/prop/yandex_storage_object_object_lock_retain_until_date">
    <rdfs:label>object_lock_retain_until_date</rdfs:label>
    <rdfs:comment>Specifies date and time in RTC3339 format until which an object is to be locked. It must be set simultaneously with `object_lock_mode`. Requires `object_lock_configuration` to be enabled on a bucket.</rdfs:comment>
    <rdfs:domain rdf:resource="http://example.org/onto/class/yandex_storage_object"/>
    <rdfs:range rdf:resource="http://www.w3.org/2001/XMLSchema#string"/>
  </owl:DatatypeProperty>
  <owl:DatatypeProperty rdf:about="http://example.org/onto/prop/yandex_storage_object_secret_key">
    <rdfs:label>secret_key</rdfs:label>
    <rdfs:comment>The secret key to use when applying changes. This value can also be provided as `storage_secret_key` specified in provider config (explicitly or within `shared_credentials_file`) is used.</rdfs:comment>
    <rdfs:domain rdf:resource="http://example.org/onto/class/yandex_storage_object"/>
    <rdfs:range rdf:resource="http://www.w3.org/2001/XMLSchema#string"/>
  </owl:DatatypeProperty>
  <owl:DatatypeProperty rdf:about="http://example.org/onto/prop/yandex_storage_object_source">
    <rdfs:label>source</rdfs:label>
    <rdfs:comment>The path to a file that will be read and uploaded as raw bytes for the object content. Conflicts with `content` and `content_base64`.</rdfs:comment>
    <rdfs:domain rdf:resource="http://example.org/onto/class/yandex_storage_object"/>
    <rdfs:range rdf:resource="http://www.w3.org/2001/XMLSchema#string"/>
  </owl:DatatypeProperty>
  <owl:DatatypeProperty rdf:about="http://example.org/onto/prop/yandex_storage_object_source_hash">
    <rdfs:label>source_hash</rdfs:label>
    <rdfs:comment>Used to trigger object update when the source content changes. So the only meaningful value is `filemd5("path/to/source"). The value is only stored in state and not saved by Yandex Storage.</rdfs:comment>
    <rdfs:domain rdf:resource="http://example.org/onto/class/yandex_storage_object"/>
    <rdfs:range rdf:resource="http://www.w3.org/2001/XMLSchema#string"/>
  </owl:DatatypeProperty>
  <owl:DatatypeProperty rdf:about="http://example.org/onto/prop/yandex_storage_object_tags">
    <rdfs:label>tags</rdfs:label>
    <rdfs:comment>The `tags` object for setting tags (or labels) for bucket. See [Tags](https://yandex.cloud/docs/storage/concepts/tags) for more information.</rdfs:comment>
    <rdfs:domain rdf:resource="http://example.org/onto/class/yandex_storage_object"/>
    <rdfs:range rdf:resource="http://www.w3.org/2001/XMLSchema#string"/>
  </owl:DatatypeProperty>
</rdf:RDF>
