<?xml version="1.0" encoding="UTF-8"?>
<rdf:RDF
  xmlns:rdf="http://www.w3.org/1999/02/22-rdf-syntax-ns#"
  xmlns:rdfs="http://www.w3.org/2000/01/rdf-schema#"
  xmlns:owl="http://www.w3.org/2002/07/owl#"
  xmlns:xsd="http://www.w3.org/2001/XMLSchema#"
  xml:base="http://example.org/onto/">
  <owl:Class rdf:about="http://example.org/onto/class/yandex_mdb_kafka_topic">
    <rdfs:label>yandex_mdb_kafka_topic</rdfs:label>
    <rdfs:comment>Manages a topic of a Kafka Topic within the Yandex Cloud. For more information, see [the official documentation](https://yandex.cloud/docs/managed-kafka/concepts).</rdfs:comment>
  </owl:Class>
  <owl:DatatypeProperty rdf:about="http://example.org/onto/prop/yandex_mdb_kafka_topic_cluster_id">
    <rdfs:label>cluster_id</rdfs:label>
    <rdfs:comment>The ID of the Kafka cluster.</rdfs:comment>
    <rdfs:domain rdf:resource="http://example.org/onto/class/yandex_mdb_kafka_topic"/>
    <rdfs:range rdf:resource="http://www.w3.org/2001/XMLSchema#string"/>
  </owl:DatatypeProperty>
  <owl:DatatypeProperty rdf:about="http://example.org/onto/prop/yandex_mdb_kafka_topic_id">
    <rdfs:label>id</rdfs:label>
    <rdfs:domain rdf:resource="http://example.org/onto/class/yandex_mdb_kafka_topic"/>
    <rdfs:range rdf:resource="http://www.w3.org/2001/XMLSchema#string"/>
  </owl:DatatypeProperty>
  <owl:DatatypeProperty rdf:about="http://example.org/onto/prop/yandex_mdb_kafka_topic_name">
    <rdfs:label>name</rdfs:label>
    <rdfs:comment>The resource name.</rdfs:comment>
    <rdfs:domain rdf:resource="http://example.org/onto/class/yandex_mdb_kafka_topic"/>
    <rdfs:range rdf:resource="http://www.w3.org/2001/XMLSchema#string"/>
  </owl:DatatypeProperty>
  <owl:DatatypeProperty rdf:about="http://example.org/onto/prop/yandex_mdb_kafka_topic_partitions">
    <rdfs:label>partitions</rdfs:label>
    <rdfs:comment>The number of the topic's partitions.</rdfs:comment>
    <rdfs:domain rdf:resource="http://example.org/onto/class/yandex_mdb_kafka_topic"/>
    <rdfs:range rdf:resource="http://www.w3.org/2001/XMLSchema#string"/>
  </owl:DatatypeProperty>
  <owl:DatatypeProperty rdf:about="http://example.org/onto/prop/yandex_mdb_kafka_topic_replication_factor">
    <rdfs:label>replication_factor</rdfs:label>
    <rdfs:comment>Amount of data copies (replicas) for the topic in the cluster.</rdfs:comment>
    <rdfs:domain rdf:resource="http://example.org/onto/class/yandex_mdb_kafka_topic"/>
    <rdfs:range rdf:resource="http://www.w3.org/2001/XMLSchema#string"/>
  </owl:DatatypeProperty>
  <owl:DatatypeProperty rdf:about="http://example.org/onto/prop/yandex_mdb_kafka_topic_create">
    <rdfs:label>create</rdfs:label>
    <rdfs:domain rdf:resource="http://example.org/onto/class/yandex_mdb_kafka_topic"/>
    <rdfs:range rdf:resource="http://www.w3.org/2001/XMLSchema#string"/>
  </owl:DatatypeProperty>
  <owl:DatatypeProperty rdf:about="http://example.org/onto/prop/yandex_mdb_kafka_topic_delete">
    <rdfs:label>delete</rdfs:label>
    <rdfs:domain rdf:resource="http://example.org/onto/class/yandex_mdb_kafka_topic"/>
    <rdfs:range rdf:resource="http://www.w3.org/2001/XMLSchema#string"/>
  </owl:DatatypeProperty>
  <owl:DatatypeProperty rdf:about="http://example.org/onto/prop/yandex_mdb_kafka_topic_read">
    <rdfs:label>read</rdfs:label>
    <rdfs:domain rdf:resource="http://example.org/onto/class/yandex_mdb_kafka_topic"/>
    <rdfs:range rdf:resource="http://www.w3.org/2001/XMLSchema#string"/>
  </owl:DatatypeProperty>
  <owl:DatatypeProperty rdf:about="http://example.org/onto/prop/yandex_mdb_kafka_topic_update">
    <rdfs:label>update</rdfs:label>
    <rdfs:domain rdf:resource="http://example.org/onto/class/yandex_mdb_kafka_topic"/>
    <rdfs:range rdf:resource="http://www.w3.org/2001/XMLSchema#string"/>
  </owl:DatatypeProperty>
  <owl:DatatypeProperty rdf:about="http://example.org/onto/prop/yandex_mdb_kafka_topic_cleanup_policy">
    <rdfs:label>cleanup_policy</rdfs:label>
    <rdfs:comment>Retention policy to use on log segments.</rdfs:comment>
    <rdfs:domain rdf:resource="http://example.org/onto/class/yandex_mdb_kafka_topic"/>
    <rdfs:range rdf:resource="http://www.w3.org/2001/XMLSchema#string"/>
  </owl:DatatypeProperty>
  <owl:DatatypeProperty rdf:about="http://example.org/onto/prop/yandex_mdb_kafka_topic_compression_type">
    <rdfs:label>compression_type</rdfs:label>
    <rdfs:comment>Compression type of kafka topic.</rdfs:comment>
    <rdfs:domain rdf:resource="http://example.org/onto/class/yandex_mdb_kafka_topic"/>
    <rdfs:range rdf:resource="http://www.w3.org/2001/XMLSchema#string"/>
  </owl:DatatypeProperty>
  <owl:DatatypeProperty rdf:about="http://example.org/onto/prop/yandex_mdb_kafka_topic_delete_retention_ms">
    <rdfs:label>delete_retention_ms</rdfs:label>
    <rdfs:comment>The amount of time to retain delete tombstone markers for log compacted topics.</rdfs:comment>
    <rdfs:domain rdf:resource="http://example.org/onto/class/yandex_mdb_kafka_topic"/>
    <rdfs:range rdf:resource="http://www.w3.org/2001/XMLSchema#string"/>
  </owl:DatatypeProperty>
  <owl:DatatypeProperty rdf:about="http://example.org/onto/prop/yandex_mdb_kafka_topic_file_delete_delay_ms">
    <rdfs:label>file_delete_delay_ms</rdfs:label>
    <rdfs:comment>The time to wait before deleting a file from the filesystem.</rdfs:comment>
    <rdfs:domain rdf:resource="http://example.org/onto/class/yandex_mdb_kafka_topic"/>
    <rdfs:range rdf:resource="http://www.w3.org/2001/XMLSchema#string"/>
  </owl:DatatypeProperty>
  <owl:DatatypeProperty rdf:about="http://example.org/onto/prop/yandex_mdb_kafka_topic_flush_messages">
    <rdfs:label>flush_messages</rdfs:label>
    <rdfs:comment>This setting allows specifying an interval at which we will force an fsync of data written to the log.</rdfs:comment>
    <rdfs:domain rdf:resource="http://example.org/onto/class/yandex_mdb_kafka_topic"/>
    <rdfs:range rdf:resource="http://www.w3.org/2001/XMLSchema#string"/>
  </owl:DatatypeProperty>
  <owl:DatatypeProperty rdf:about="http://example.org/onto/prop/yandex_mdb_kafka_topic_flush_ms">
    <rdfs:label>flush_ms</rdfs:label>
    <rdfs:comment>This setting allows specifying a time interval at which we will force an fsync of data written to the log.</rdfs:comment>
    <rdfs:domain rdf:resource="http://example.org/onto/class/yandex_mdb_kafka_topic"/>
    <rdfs:range rdf:resource="http://www.w3.org/2001/XMLSchema#string"/>
  </owl:DatatypeProperty>
  <owl:DatatypeProperty rdf:about="http://example.org/onto/prop/yandex_mdb_kafka_topic_max_message_bytes">
    <rdfs:label>max_message_bytes</rdfs:label>
    <rdfs:comment>The largest record batch size allowed by Kafka (after compression if compression is enabled).</rdfs:comment>
    <rdfs:domain rdf:resource="http://example.org/onto/class/yandex_mdb_kafka_topic"/>
    <rdfs:range rdf:resource="http://www.w3.org/2001/XMLSchema#string"/>
  </owl:DatatypeProperty>
  <owl:DatatypeProperty rdf:about="http://example.org/onto/prop/yandex_mdb_kafka_topic_min_compaction_lag_ms">
    <rdfs:label>min_compaction_lag_ms</rdfs:label>
    <rdfs:comment>The minimum time a message will remain uncompacted in the log. Only applicable for logs that are being compacted.</rdfs:comment>
    <rdfs:domain rdf:resource="http://example.org/onto/class/yandex_mdb_kafka_topic"/>
    <rdfs:range rdf:resource="http://www.w3.org/2001/XMLSchema#string"/>
  </owl:DatatypeProperty>
  <owl:DatatypeProperty rdf:about="http://example.org/onto/prop/yandex_mdb_kafka_topic_min_insync_replicas">
    <rdfs:label>min_insync_replicas</rdfs:label>
    <rdfs:comment>When a producer sets acks to "all" (or "-1"), this configuration specifies the minimum number of replicas that must acknowledge a write for the write to be considered successful.</rdfs:comment>
    <rdfs:domain rdf:resource="http://example.org/onto/class/yandex_mdb_kafka_topic"/>
    <rdfs:range rdf:resource="http://www.w3.org/2001/XMLSchema#string"/>
  </owl:DatatypeProperty>
  <owl:DatatypeProperty rdf:about="http://example.org/onto/prop/yandex_mdb_kafka_topic_preallocate">
    <rdfs:label>preallocate</rdfs:label>
    <rdfs:comment>True if we should preallocate the file on disk when creating a new log segment.</rdfs:comment>
    <rdfs:domain rdf:resource="http://example.org/onto/class/yandex_mdb_kafka_topic"/>
    <rdfs:range rdf:resource="http://www.w3.org/2001/XMLSchema#string"/>
  </owl:DatatypeProperty>
  <owl:DatatypeProperty rdf:about="http://example.org/onto/prop/yandex_mdb_kafka_topic_retention_bytes">
    <rdfs:label>retention_bytes</rdfs:label>
    <rdfs:comment>This configuration controls the maximum size a partition (which consists of log segments) can grow to before we will discard old log segments to free up space if we are using the "delete" retention policy.</rdfs:comment>
    <rdfs:domain rdf:resource="http://example.org/onto/class/yandex_mdb_kafka_topic"/>
    <rdfs:range rdf:resource="http://www.w3.org/2001/XMLSchema#string"/>
  </owl:DatatypeProperty>
  <owl:DatatypeProperty rdf:about="http://example.org/onto/prop/yandex_mdb_kafka_topic_retention_ms">
    <rdfs:label>retention_ms</rdfs:label>
    <rdfs:comment>This configuration controls the maximum time we will retain a log before we will discard old log segments to free up space if we are using the "delete" retention policy.</rdfs:comment>
    <rdfs:domain rdf:resource="http://example.org/onto/class/yandex_mdb_kafka_topic"/>
    <rdfs:range rdf:resource="http://www.w3.org/2001/XMLSchema#string"/>
  </owl:DatatypeProperty>
  <owl:DatatypeProperty rdf:about="http://example.org/onto/prop/yandex_mdb_kafka_topic_segment_bytes">
    <rdfs:label>segment_bytes</rdfs:label>
    <rdfs:comment>This configuration controls the segment file size for the log.</rdfs:comment>
    <rdfs:domain rdf:resource="http://example.org/onto/class/yandex_mdb_kafka_topic"/>
    <rdfs:range rdf:resource="http://www.w3.org/2001/XMLSchema#string"/>
  </owl:DatatypeProperty>
</rdf:RDF>
