<?xml version="1.0" encoding="UTF-8"?>
<rdf:RDF
  xmlns:rdf="http://www.w3.org/1999/02/22-rdf-syntax-ns#"
  xmlns:rdfs="http://www.w3.org/2000/01/rdf-schema#"
  xmlns:owl="http://www.w3.org/2002/07/owl#"
  xmlns:xsd="http://www.w3.org/2001/XMLSchema#"
  xml:base="http://example.org/onto/">
  <owl:Class rdf:about="http://example.org/onto/class/yandex_iam_workload_identity_federated_credential">
    <rdfs:label>yandex_iam_workload_identity_federated_credential</rdfs:label>
    <rdfs:comment>A federated credential.</rdfs:comment>
  </owl:Class>
  <owl:DatatypeProperty rdf:about="http://example.org/onto/prop/yandex_iam_workload_identity_federated_credential_created_at">
    <rdfs:label>created_at</rdfs:label>
    <rdfs:comment>Creation timestamp.</rdfs:comment>
    <rdfs:domain rdf:resource="http://example.org/onto/class/yandex_iam_workload_identity_federated_credential"/>
    <rdfs:range rdf:resource="http://www.w3.org/2001/XMLSchema#string"/>
  </owl:DatatypeProperty>
  <owl:DatatypeProperty rdf:about="http://example.org/onto/prop/yandex_iam_workload_identity_federated_credential_external_subject_id">
    <rdfs:label>external_subject_id</rdfs:label>
    <rdfs:comment>Id of the external subject.</rdfs:comment>
    <rdfs:domain rdf:resource="http://example.org/onto/class/yandex_iam_workload_identity_federated_credential"/>
    <rdfs:range rdf:resource="http://www.w3.org/2001/XMLSchema#string"/>
  </owl:DatatypeProperty>
  <owl:DatatypeProperty rdf:about="http://example.org/onto/prop/yandex_iam_workload_identity_federated_credential_federated_credential_id">
    <rdfs:label>federated_credential_id</rdfs:label>
    <rdfs:comment>ID of the federated credential to return.
 To get the federated credential ID, make a [FederatedCredentialService.List] request.</rdfs:comment>
    <rdfs:domain rdf:resource="http://example.org/onto/class/yandex_iam_workload_identity_federated_credential"/>
    <rdfs:range rdf:resource="http://www.w3.org/2001/XMLSchema#string"/>
  </owl:DatatypeProperty>
  <owl:DatatypeProperty rdf:about="http://example.org/onto/prop/yandex_iam_workload_identity_federated_credential_federation_id">
    <rdfs:label>federation_id</rdfs:label>
    <rdfs:comment>ID of the workload identity federation which is used for authentication.</rdfs:comment>
    <rdfs:domain rdf:resource="http://example.org/onto/class/yandex_iam_workload_identity_federated_credential"/>
    <rdfs:range rdf:resource="http://www.w3.org/2001/XMLSchema#string"/>
  </owl:DatatypeProperty>
  <owl:DatatypeProperty rdf:about="http://example.org/onto/prop/yandex_iam_workload_identity_federated_credential_id">
    <rdfs:label>id</rdfs:label>
    <rdfs:comment>ID of the federated credential to return.
 To get the federated credential ID, make a [FederatedCredentialService.List] request.</rdfs:comment>
    <rdfs:domain rdf:resource="http://example.org/onto/class/yandex_iam_workload_identity_federated_credential"/>
    <rdfs:range rdf:resource="http://www.w3.org/2001/XMLSchema#string"/>
  </owl:DatatypeProperty>
  <owl:DatatypeProperty rdf:about="http://example.org/onto/prop/yandex_iam_workload_identity_federated_credential_service_account_id">
    <rdfs:label>service_account_id</rdfs:label>
    <rdfs:comment>Id of the service account that the federated credential belongs to.</rdfs:comment>
    <rdfs:domain rdf:resource="http://example.org/onto/class/yandex_iam_workload_identity_federated_credential"/>
    <rdfs:range rdf:resource="http://www.w3.org/2001/XMLSchema#string"/>
  </owl:DatatypeProperty>
  <owl:DatatypeProperty rdf:about="http://example.org/onto/prop/yandex_iam_workload_identity_federated_credential_create">
    <rdfs:label>create</rdfs:label>
    <rdfs:comment>A string that can be [parsed as a duration](https://pkg.go.dev/time#ParseDuration) consisting of numbers and unit suffixes, such as "30s" or "2h45m". Valid time units are "s" (seconds), "m" (minutes), "h" (hours).</rdfs:comment>
    <rdfs:domain rdf:resource="http://example.org/onto/class/yandex_iam_workload_identity_federated_credential"/>
    <rdfs:range rdf:resource="http://www.w3.org/2001/XMLSchema#string"/>
  </owl:DatatypeProperty>
  <owl:DatatypeProperty rdf:about="http://example.org/onto/prop/yandex_iam_workload_identity_federated_credential_delete">
    <rdfs:label>delete</rdfs:label>
    <rdfs:comment>A string that can be [parsed as a duration](https://pkg.go.dev/time#ParseDuration) consisting of numbers and unit suffixes, such as "30s" or "2h45m". Valid time units are "s" (seconds), "m" (minutes), "h" (hours). Setting a timeout for a Delete operation is only applicable if changes are saved into state before the destroy operation occurs.</rdfs:comment>
    <rdfs:domain rdf:resource="http://example.org/onto/class/yandex_iam_workload_identity_federated_credential"/>
    <rdfs:range rdf:resource="http://www.w3.org/2001/XMLSchema#string"/>
  </owl:DatatypeProperty>
  <owl:DatatypeProperty rdf:about="http://example.org/onto/prop/yandex_iam_workload_identity_federated_credential_read">
    <rdfs:label>read</rdfs:label>
    <rdfs:comment>A string that can be [parsed as a duration](https://pkg.go.dev/time#ParseDuration) consisting of numbers and unit suffixes, such as "30s" or "2h45m". Valid time units are "s" (seconds), "m" (minutes), "h" (hours). Read operations occur during any refresh or planning operation when refresh is enabled.</rdfs:comment>
    <rdfs:domain rdf:resource="http://example.org/onto/class/yandex_iam_workload_identity_federated_credential"/>
    <rdfs:range rdf:resource="http://www.w3.org/2001/XMLSchema#string"/>
  </owl:DatatypeProperty>
  <owl:DatatypeProperty rdf:about="http://example.org/onto/prop/yandex_iam_workload_identity_federated_credential_update">
    <rdfs:label>update</rdfs:label>
    <rdfs:comment>A string that can be [parsed as a duration](https://pkg.go.dev/time#ParseDuration) consisting of numbers and unit suffixes, such as "30s" or "2h45m". Valid time units are "s" (seconds), "m" (minutes), "h" (hours).</rdfs:comment>
    <rdfs:domain rdf:resource="http://example.org/onto/class/yandex_iam_workload_identity_federated_credential"/>
    <rdfs:range rdf:resource="http://www.w3.org/2001/XMLSchema#string"/>
  </owl:DatatypeProperty>
</rdf:RDF>
