<?xml version="1.0" encoding="UTF-8"?>
<rdf:RDF
  xmlns:rdf="http://www.w3.org/1999/02/22-rdf-syntax-ns#"
  xmlns:rdfs="http://www.w3.org/2000/01/rdf-schema#"
  xmlns:owl="http://www.w3.org/2002/07/owl#"
  xmlns:xsd="http://www.w3.org/2001/XMLSchema#"
  xml:base="http://example.org/onto/">
  <owl:Class rdf:about="http://example.org/onto/class/yandex_iam_service_account_static_access_key">
    <rdfs:label>yandex_iam_service_account_static_access_key</rdfs:label>
    <rdfs:comment>Allows management of [Yandex Cloud IAM service account static access keys](https://yandex.cloud/docs/iam/operations/sa/create-access-key). Generated pair of keys is used to access [Yandex Object Storage](https://yandex.cloud/docs/storage) on behalf of service account.

Before using keys do not forget to [assign a proper role](https://yandex.cloud/docs/iam/operations/sa/assign-role-for-sa) to the service account.</rdfs:comment>
  </owl:Class>
  <owl:DatatypeProperty rdf:about="http://example.org/onto/prop/yandex_iam_service_account_static_access_key_access_key">
    <rdfs:label>access_key</rdfs:label>
    <rdfs:comment>ID of the static access key. This is only populated when `output_to_lockbox` is not provided.</rdfs:comment>
    <rdfs:domain rdf:resource="http://example.org/onto/class/yandex_iam_service_account_static_access_key"/>
    <rdfs:range rdf:resource="http://www.w3.org/2001/XMLSchema#string"/>
  </owl:DatatypeProperty>
  <owl:DatatypeProperty rdf:about="http://example.org/onto/prop/yandex_iam_service_account_static_access_key_created_at">
    <rdfs:label>created_at</rdfs:label>
    <rdfs:comment>The creation timestamp of the resource.</rdfs:comment>
    <rdfs:domain rdf:resource="http://example.org/onto/class/yandex_iam_service_account_static_access_key"/>
    <rdfs:range rdf:resource="http://www.w3.org/2001/XMLSchema#string"/>
  </owl:DatatypeProperty>
  <owl:DatatypeProperty rdf:about="http://example.org/onto/prop/yandex_iam_service_account_static_access_key_description">
    <rdfs:label>description</rdfs:label>
    <rdfs:comment>The resource description.</rdfs:comment>
    <rdfs:domain rdf:resource="http://example.org/onto/class/yandex_iam_service_account_static_access_key"/>
    <rdfs:range rdf:resource="http://www.w3.org/2001/XMLSchema#string"/>
  </owl:DatatypeProperty>
  <owl:DatatypeProperty rdf:about="http://example.org/onto/prop/yandex_iam_service_account_static_access_key_encrypted_secret_key">
    <rdfs:label>encrypted_secret_key</rdfs:label>
    <rdfs:comment>The encrypted secret, base64 encoded. This is only populated when `pgp_key` is supplied.</rdfs:comment>
    <rdfs:domain rdf:resource="http://example.org/onto/class/yandex_iam_service_account_static_access_key"/>
    <rdfs:range rdf:resource="http://www.w3.org/2001/XMLSchema#string"/>
  </owl:DatatypeProperty>
  <owl:DatatypeProperty rdf:about="http://example.org/onto/prop/yandex_iam_service_account_static_access_key_id">
    <rdfs:label>id</rdfs:label>
    <rdfs:domain rdf:resource="http://example.org/onto/class/yandex_iam_service_account_static_access_key"/>
    <rdfs:range rdf:resource="http://www.w3.org/2001/XMLSchema#string"/>
  </owl:DatatypeProperty>
  <owl:DatatypeProperty rdf:about="http://example.org/onto/prop/yandex_iam_service_account_static_access_key_key_fingerprint">
    <rdfs:label>key_fingerprint</rdfs:label>
    <rdfs:comment>The fingerprint of the PGP key used to encrypt the secret key. This is only populated when `pgp_key` is supplied.</rdfs:comment>
    <rdfs:domain rdf:resource="http://example.org/onto/class/yandex_iam_service_account_static_access_key"/>
    <rdfs:range rdf:resource="http://www.w3.org/2001/XMLSchema#string"/>
  </owl:DatatypeProperty>
  <owl:DatatypeProperty rdf:about="http://example.org/onto/prop/yandex_iam_service_account_static_access_key_output_to_lockbox_version_id">
    <rdfs:label>output_to_lockbox_version_id</rdfs:label>
    <rdfs:comment>ID of the Lockbox secret version that contains the value of `secret_key`. This is only populated when `output_to_lockbox` is supplied. This version will be destroyed when the IAM key is destroyed, or when `output_to_lockbox` is removed.</rdfs:comment>
    <rdfs:domain rdf:resource="http://example.org/onto/class/yandex_iam_service_account_static_access_key"/>
    <rdfs:range rdf:resource="http://www.w3.org/2001/XMLSchema#string"/>
  </owl:DatatypeProperty>
  <owl:DatatypeProperty rdf:about="http://example.org/onto/prop/yandex_iam_service_account_static_access_key_pgp_key">
    <rdfs:label>pgp_key</rdfs:label>
    <rdfs:comment>An optional PGP key to encrypt the resulting secret key material. May either be a base64-encoded public key or a keybase username in the form `keybase:keybaseusername`.</rdfs:comment>
    <rdfs:domain rdf:resource="http://example.org/onto/class/yandex_iam_service_account_static_access_key"/>
    <rdfs:range rdf:resource="http://www.w3.org/2001/XMLSchema#string"/>
  </owl:DatatypeProperty>
  <owl:DatatypeProperty rdf:about="http://example.org/onto/prop/yandex_iam_service_account_static_access_key_secret_key">
    <rdfs:label>secret_key</rdfs:label>
    <rdfs:comment>Private part of generated static access key. This is only populated when neither `pgp_key` nor `output_to_lockbox` are provided.</rdfs:comment>
    <rdfs:domain rdf:resource="http://example.org/onto/class/yandex_iam_service_account_static_access_key"/>
    <rdfs:range rdf:resource="http://www.w3.org/2001/XMLSchema#string"/>
  </owl:DatatypeProperty>
  <owl:DatatypeProperty rdf:about="http://example.org/onto/prop/yandex_iam_service_account_static_access_key_service_account_id">
    <rdfs:label>service_account_id</rdfs:label>
    <rdfs:comment>ID of the service account which is used to get a static key.</rdfs:comment>
    <rdfs:domain rdf:resource="http://example.org/onto/class/yandex_iam_service_account_static_access_key"/>
    <rdfs:range rdf:resource="http://www.w3.org/2001/XMLSchema#string"/>
  </owl:DatatypeProperty>
  <owl:DatatypeProperty rdf:about="http://example.org/onto/prop/yandex_iam_service_account_static_access_key_entry_for_access_key">
    <rdfs:label>entry_for_access_key</rdfs:label>
    <rdfs:comment>entry that will store the value of access_key</rdfs:comment>
    <rdfs:domain rdf:resource="http://example.org/onto/class/yandex_iam_service_account_static_access_key"/>
    <rdfs:range rdf:resource="http://www.w3.org/2001/XMLSchema#string"/>
  </owl:DatatypeProperty>
  <owl:DatatypeProperty rdf:about="http://example.org/onto/prop/yandex_iam_service_account_static_access_key_entry_for_secret_key">
    <rdfs:label>entry_for_secret_key</rdfs:label>
    <rdfs:comment>entry that will store the value of secret_key</rdfs:comment>
    <rdfs:domain rdf:resource="http://example.org/onto/class/yandex_iam_service_account_static_access_key"/>
    <rdfs:range rdf:resource="http://www.w3.org/2001/XMLSchema#string"/>
  </owl:DatatypeProperty>
  <owl:DatatypeProperty rdf:about="http://example.org/onto/prop/yandex_iam_service_account_static_access_key_secret_id">
    <rdfs:label>secret_id</rdfs:label>
    <rdfs:comment>ID of the Lockbox secret where to store the sensible values.</rdfs:comment>
    <rdfs:domain rdf:resource="http://example.org/onto/class/yandex_iam_service_account_static_access_key"/>
    <rdfs:range rdf:resource="http://www.w3.org/2001/XMLSchema#string"/>
  </owl:DatatypeProperty>
</rdf:RDF>
