<?xml version="1.0" encoding="UTF-8"?>
<rdf:RDF
  xmlns:rdf="http://www.w3.org/1999/02/22-rdf-syntax-ns#"
  xmlns:rdfs="http://www.w3.org/2000/01/rdf-schema#"
  xmlns:owl="http://www.w3.org/2002/07/owl#"
  xmlns:xsd="http://www.w3.org/2001/XMLSchema#"
  xml:base="http://example.org/onto/">
  <owl:Class rdf:about="http://example.org/onto/class/yandex_connectionmanager_connection">
    <rdfs:label>yandex_connectionmanager_connection</rdfs:label>
    <rdfs:comment>A generic empty message that you can re-use to avoid defining duplicated
 empty messages in your APIs. A typical example is to use it as the request
 or the response type of an API method. For instance:

     service Foo {
       rpc Bar(google.protobuf.Empty) returns (google.protobuf.Empty);
     }</rdfs:comment>
  </owl:Class>
  <owl:DatatypeProperty rdf:about="http://example.org/onto/prop/yandex_connectionmanager_connection_can_use">
    <rdfs:label>can_use</rdfs:label>
    <rdfs:comment>package: yandex.cloud.connectionmanager.v1
filename: yandex/cloud/connectionmanager/v1/connection.proto</rdfs:comment>
    <rdfs:domain rdf:resource="http://example.org/onto/class/yandex_connectionmanager_connection"/>
    <rdfs:range rdf:resource="http://www.w3.org/2001/XMLSchema#string"/>
  </owl:DatatypeProperty>
  <owl:DatatypeProperty rdf:about="http://example.org/onto/prop/yandex_connectionmanager_connection_connection_id">
    <rdfs:label>connection_id</rdfs:label>
    <rdfs:comment>package: yandex.cloud.connectionmanager.v1
filename: yandex/cloud/connectionmanager/v1/connection_service.proto</rdfs:comment>
    <rdfs:domain rdf:resource="http://example.org/onto/class/yandex_connectionmanager_connection"/>
    <rdfs:range rdf:resource="http://www.w3.org/2001/XMLSchema#string"/>
  </owl:DatatypeProperty>
  <owl:DatatypeProperty rdf:about="http://example.org/onto/prop/yandex_connectionmanager_connection_created_at">
    <rdfs:label>created_at</rdfs:label>
    <rdfs:comment>package: yandex.cloud.connectionmanager.v1
filename: yandex/cloud/connectionmanager/v1/connection.proto</rdfs:comment>
    <rdfs:domain rdf:resource="http://example.org/onto/class/yandex_connectionmanager_connection"/>
    <rdfs:range rdf:resource="http://www.w3.org/2001/XMLSchema#string"/>
  </owl:DatatypeProperty>
  <owl:DatatypeProperty rdf:about="http://example.org/onto/prop/yandex_connectionmanager_connection_created_by">
    <rdfs:label>created_by</rdfs:label>
    <rdfs:comment>package: yandex.cloud.connectionmanager.v1
filename: yandex/cloud/connectionmanager/v1/connection.proto</rdfs:comment>
    <rdfs:domain rdf:resource="http://example.org/onto/class/yandex_connectionmanager_connection"/>
    <rdfs:range rdf:resource="http://www.w3.org/2001/XMLSchema#string"/>
  </owl:DatatypeProperty>
  <owl:DatatypeProperty rdf:about="http://example.org/onto/prop/yandex_connectionmanager_connection_description">
    <rdfs:label>description</rdfs:label>
    <rdfs:comment>package: yandex.cloud.connectionmanager.v1
filename: yandex/cloud/connectionmanager/v1/connection.proto</rdfs:comment>
    <rdfs:domain rdf:resource="http://example.org/onto/class/yandex_connectionmanager_connection"/>
    <rdfs:range rdf:resource="http://www.w3.org/2001/XMLSchema#string"/>
  </owl:DatatypeProperty>
  <owl:DatatypeProperty rdf:about="http://example.org/onto/prop/yandex_connectionmanager_connection_folder_id">
    <rdfs:label>folder_id</rdfs:label>
    <rdfs:comment>package: yandex.cloud.connectionmanager.v1
filename: yandex/cloud/connectionmanager/v1/connection.proto</rdfs:comment>
    <rdfs:domain rdf:resource="http://example.org/onto/class/yandex_connectionmanager_connection"/>
    <rdfs:range rdf:resource="http://www.w3.org/2001/XMLSchema#string"/>
  </owl:DatatypeProperty>
  <owl:DatatypeProperty rdf:about="http://example.org/onto/prop/yandex_connectionmanager_connection_id">
    <rdfs:label>id</rdfs:label>
    <rdfs:comment>package: yandex.cloud.connectionmanager.v1
filename: yandex/cloud/connectionmanager/v1/connection_service.proto</rdfs:comment>
    <rdfs:domain rdf:resource="http://example.org/onto/class/yandex_connectionmanager_connection"/>
    <rdfs:range rdf:resource="http://www.w3.org/2001/XMLSchema#string"/>
  </owl:DatatypeProperty>
  <owl:DatatypeProperty rdf:about="http://example.org/onto/prop/yandex_connectionmanager_connection_is_managed">
    <rdfs:label>is_managed</rdfs:label>
    <rdfs:comment>package: yandex.cloud.connectionmanager.v1
filename: yandex/cloud/connectionmanager/v1/connection.proto</rdfs:comment>
    <rdfs:domain rdf:resource="http://example.org/onto/class/yandex_connectionmanager_connection"/>
    <rdfs:range rdf:resource="http://www.w3.org/2001/XMLSchema#string"/>
  </owl:DatatypeProperty>
  <owl:DatatypeProperty rdf:about="http://example.org/onto/prop/yandex_connectionmanager_connection_labels">
    <rdfs:label>labels</rdfs:label>
    <rdfs:comment>package: yandex.cloud.connectionmanager.v1
filename: yandex/cloud/connectionmanager/v1/connection.proto</rdfs:comment>
    <rdfs:domain rdf:resource="http://example.org/onto/class/yandex_connectionmanager_connection"/>
    <rdfs:range rdf:resource="http://www.w3.org/2001/XMLSchema#string"/>
  </owl:DatatypeProperty>
  <owl:DatatypeProperty rdf:about="http://example.org/onto/prop/yandex_connectionmanager_connection_lockbox_secret">
    <rdfs:label>lockbox_secret</rdfs:label>
    <rdfs:comment>package: yandex.cloud.connectionmanager.v1
filename: yandex/cloud/connectionmanager/v1/connection.proto</rdfs:comment>
    <rdfs:domain rdf:resource="http://example.org/onto/class/yandex_connectionmanager_connection"/>
    <rdfs:range rdf:resource="http://www.w3.org/2001/XMLSchema#string"/>
  </owl:DatatypeProperty>
  <owl:DatatypeProperty rdf:about="http://example.org/onto/prop/yandex_connectionmanager_connection_name">
    <rdfs:label>name</rdfs:label>
    <rdfs:comment>package: yandex.cloud.connectionmanager.v1
filename: yandex/cloud/connectionmanager/v1/connection.proto</rdfs:comment>
    <rdfs:domain rdf:resource="http://example.org/onto/class/yandex_connectionmanager_connection"/>
    <rdfs:range rdf:resource="http://www.w3.org/2001/XMLSchema#string"/>
  </owl:DatatypeProperty>
  <owl:DatatypeProperty rdf:about="http://example.org/onto/prop/yandex_connectionmanager_connection_params">
    <rdfs:label>params</rdfs:label>
    <rdfs:comment>package: yandex.cloud.connectionmanager.v1
filename: yandex/cloud/connectionmanager/v1/connection.proto</rdfs:comment>
    <rdfs:domain rdf:resource="http://example.org/onto/class/yandex_connectionmanager_connection"/>
    <rdfs:range rdf:resource="http://www.w3.org/2001/XMLSchema#string"/>
  </owl:DatatypeProperty>
  <owl:DatatypeProperty rdf:about="http://example.org/onto/prop/yandex_connectionmanager_connection_timeouts">
    <rdfs:label>timeouts</rdfs:label>
    <rdfs:domain rdf:resource="http://example.org/onto/class/yandex_connectionmanager_connection"/>
    <rdfs:range rdf:resource="http://www.w3.org/2001/XMLSchema#string"/>
  </owl:DatatypeProperty>
  <owl:DatatypeProperty rdf:about="http://example.org/onto/prop/yandex_connectionmanager_connection_updated_at">
    <rdfs:label>updated_at</rdfs:label>
    <rdfs:comment>package: yandex.cloud.connectionmanager.v1
filename: yandex/cloud/connectionmanager/v1/connection.proto</rdfs:comment>
    <rdfs:domain rdf:resource="http://example.org/onto/class/yandex_connectionmanager_connection"/>
    <rdfs:range rdf:resource="http://www.w3.org/2001/XMLSchema#string"/>
  </owl:DatatypeProperty>
</rdf:RDF>
