<?xml version="1.0" encoding="UTF-8"?>
<rdf:RDF
  xmlns:rdf="http://www.w3.org/1999/02/22-rdf-syntax-ns#"
  xmlns:rdfs="http://www.w3.org/2000/01/rdf-schema#"
  xmlns:owl="http://www.w3.org/2002/07/owl#"
  xmlns:xsd="http://www.w3.org/2001/XMLSchema#"
  xml:base="http://example.org/onto/">
  <owl:Class rdf:about="http://example.org/onto/class/yandex_compute_disk_placement_group">
    <rdfs:label>yandex_compute_disk_placement_group</rdfs:label>
  </owl:Class>
  <owl:DatatypeProperty rdf:about="http://example.org/onto/prop/yandex_compute_disk_placement_group_created_at">
    <rdfs:label>created_at</rdfs:label>
    <rdfs:comment>Creation timestamp in [RFC3339](https://www.ietf.org/rfc/rfc3339.txt) text format.</rdfs:comment>
    <rdfs:domain rdf:resource="http://example.org/onto/class/yandex_compute_disk_placement_group"/>
    <rdfs:range rdf:resource="http://www.w3.org/2001/XMLSchema#string"/>
  </owl:DatatypeProperty>
  <owl:DatatypeProperty rdf:about="http://example.org/onto/prop/yandex_compute_disk_placement_group_description">
    <rdfs:label>description</rdfs:label>
    <rdfs:comment>Description of the placement group.</rdfs:comment>
    <rdfs:domain rdf:resource="http://example.org/onto/class/yandex_compute_disk_placement_group"/>
    <rdfs:range rdf:resource="http://www.w3.org/2001/XMLSchema#string"/>
  </owl:DatatypeProperty>
  <owl:DatatypeProperty rdf:about="http://example.org/onto/prop/yandex_compute_disk_placement_group_disk_placement_group_id">
    <rdfs:label>disk_placement_group_id</rdfs:label>
    <rdfs:comment>ID of the placement group to return.
 To get the placement group ID, use [DiskPlacementGroupService.List] request.</rdfs:comment>
    <rdfs:domain rdf:resource="http://example.org/onto/class/yandex_compute_disk_placement_group"/>
    <rdfs:range rdf:resource="http://www.w3.org/2001/XMLSchema#string"/>
  </owl:DatatypeProperty>
  <owl:DatatypeProperty rdf:about="http://example.org/onto/prop/yandex_compute_disk_placement_group_folder_id">
    <rdfs:label>folder_id</rdfs:label>
    <rdfs:comment>ID of the folder that the placement group belongs to.</rdfs:comment>
    <rdfs:domain rdf:resource="http://example.org/onto/class/yandex_compute_disk_placement_group"/>
    <rdfs:range rdf:resource="http://www.w3.org/2001/XMLSchema#string"/>
  </owl:DatatypeProperty>
  <owl:DatatypeProperty rdf:about="http://example.org/onto/prop/yandex_compute_disk_placement_group_id">
    <rdfs:label>id</rdfs:label>
    <rdfs:comment>ID of the placement group to return.
 To get the placement group ID, use [DiskPlacementGroupService.List] request.</rdfs:comment>
    <rdfs:domain rdf:resource="http://example.org/onto/class/yandex_compute_disk_placement_group"/>
    <rdfs:range rdf:resource="http://www.w3.org/2001/XMLSchema#string"/>
  </owl:DatatypeProperty>
  <owl:DatatypeProperty rdf:about="http://example.org/onto/prop/yandex_compute_disk_placement_group_labels">
    <rdfs:label>labels</rdfs:label>
    <rdfs:comment>Resource labels as `key:value` pairs.</rdfs:comment>
    <rdfs:domain rdf:resource="http://example.org/onto/class/yandex_compute_disk_placement_group"/>
    <rdfs:range rdf:resource="http://www.w3.org/2001/XMLSchema#string"/>
  </owl:DatatypeProperty>
  <owl:DatatypeProperty rdf:about="http://example.org/onto/prop/yandex_compute_disk_placement_group_name">
    <rdfs:label>name</rdfs:label>
    <rdfs:comment>Name of the placement group.
 The name is unique within the folder.</rdfs:comment>
    <rdfs:domain rdf:resource="http://example.org/onto/class/yandex_compute_disk_placement_group"/>
    <rdfs:range rdf:resource="http://www.w3.org/2001/XMLSchema#string"/>
  </owl:DatatypeProperty>
  <owl:DatatypeProperty rdf:about="http://example.org/onto/prop/yandex_compute_disk_placement_group_status">
    <rdfs:label>status</rdfs:label>
    <rdfs:comment>Current status of the placement group</rdfs:comment>
    <rdfs:domain rdf:resource="http://example.org/onto/class/yandex_compute_disk_placement_group"/>
    <rdfs:range rdf:resource="http://www.w3.org/2001/XMLSchema#string"/>
  </owl:DatatypeProperty>
  <owl:DatatypeProperty rdf:about="http://example.org/onto/prop/yandex_compute_disk_placement_group_zone">
    <rdfs:label>zone</rdfs:label>
    <rdfs:comment>ID of the availability zone where the placement group resides.</rdfs:comment>
    <rdfs:domain rdf:resource="http://example.org/onto/class/yandex_compute_disk_placement_group"/>
    <rdfs:range rdf:resource="http://www.w3.org/2001/XMLSchema#string"/>
  </owl:DatatypeProperty>
  <owl:DatatypeProperty rdf:about="http://example.org/onto/prop/yandex_compute_disk_placement_group_create">
    <rdfs:label>create</rdfs:label>
    <rdfs:comment>A string that can be [parsed as a duration](https://pkg.go.dev/time#ParseDuration) consisting of numbers and unit suffixes, such as "30s" or "2h45m". Valid time units are "s" (seconds), "m" (minutes), "h" (hours).</rdfs:comment>
    <rdfs:domain rdf:resource="http://example.org/onto/class/yandex_compute_disk_placement_group"/>
    <rdfs:range rdf:resource="http://www.w3.org/2001/XMLSchema#string"/>
  </owl:DatatypeProperty>
  <owl:DatatypeProperty rdf:about="http://example.org/onto/prop/yandex_compute_disk_placement_group_delete">
    <rdfs:label>delete</rdfs:label>
    <rdfs:comment>A string that can be [parsed as a duration](https://pkg.go.dev/time#ParseDuration) consisting of numbers and unit suffixes, such as "30s" or "2h45m". Valid time units are "s" (seconds), "m" (minutes), "h" (hours). Setting a timeout for a Delete operation is only applicable if changes are saved into state before the destroy operation occurs.</rdfs:comment>
    <rdfs:domain rdf:resource="http://example.org/onto/class/yandex_compute_disk_placement_group"/>
    <rdfs:range rdf:resource="http://www.w3.org/2001/XMLSchema#string"/>
  </owl:DatatypeProperty>
  <owl:DatatypeProperty rdf:about="http://example.org/onto/prop/yandex_compute_disk_placement_group_read">
    <rdfs:label>read</rdfs:label>
    <rdfs:comment>A string that can be [parsed as a duration](https://pkg.go.dev/time#ParseDuration) consisting of numbers and unit suffixes, such as "30s" or "2h45m". Valid time units are "s" (seconds), "m" (minutes), "h" (hours). Read operations occur during any refresh or planning operation when refresh is enabled.</rdfs:comment>
    <rdfs:domain rdf:resource="http://example.org/onto/class/yandex_compute_disk_placement_group"/>
    <rdfs:range rdf:resource="http://www.w3.org/2001/XMLSchema#string"/>
  </owl:DatatypeProperty>
  <owl:DatatypeProperty rdf:about="http://example.org/onto/prop/yandex_compute_disk_placement_group_update">
    <rdfs:label>update</rdfs:label>
    <rdfs:comment>A string that can be [parsed as a duration](https://pkg.go.dev/time#ParseDuration) consisting of numbers and unit suffixes, such as "30s" or "2h45m". Valid time units are "s" (seconds), "m" (minutes), "h" (hours).</rdfs:comment>
    <rdfs:domain rdf:resource="http://example.org/onto/class/yandex_compute_disk_placement_group"/>
    <rdfs:range rdf:resource="http://www.w3.org/2001/XMLSchema#string"/>
  </owl:DatatypeProperty>
</rdf:RDF>
