<?xml version="1.0" encoding="UTF-8"?>
<rdf:RDF
  xmlns:rdf="http://www.w3.org/1999/02/22-rdf-syntax-ns#"
  xmlns:rdfs="http://www.w3.org/2000/01/rdf-schema#"
  xmlns:owl="http://www.w3.org/2002/07/owl#"
  xmlns:xsd="http://www.w3.org/2001/XMLSchema#"
  xml:base="http://example.org/onto/">
  <owl:Class rdf:about="http://example.org/onto/class/yandex_organizationmanager_user_ssh_key">
    <rdfs:label>yandex_organizationmanager_user_ssh_key</rdfs:label>
  </owl:Class>
  <owl:DatatypeProperty rdf:about="http://example.org/onto/prop/yandex_organizationmanager_user_ssh_key_created_at">
    <rdfs:label>created_at</rdfs:label>
    <rdfs:comment>package: yandex.cloud.organizationmanager.v1
filename: yandex/cloud/organizationmanager/v1/user_ssh_key.proto</rdfs:comment>
    <rdfs:domain rdf:resource="http://example.org/onto/class/yandex_organizationmanager_user_ssh_key"/>
    <rdfs:range rdf:resource="http://www.w3.org/2001/XMLSchema#string"/>
  </owl:DatatypeProperty>
  <owl:DatatypeProperty rdf:about="http://example.org/onto/prop/yandex_organizationmanager_user_ssh_key_data">
    <rdfs:label>data</rdfs:label>
    <rdfs:comment>package: yandex.cloud.organizationmanager.v1
filename: yandex/cloud/organizationmanager/v1/user_ssh_key.proto</rdfs:comment>
    <rdfs:domain rdf:resource="http://example.org/onto/class/yandex_organizationmanager_user_ssh_key"/>
    <rdfs:range rdf:resource="http://www.w3.org/2001/XMLSchema#string"/>
  </owl:DatatypeProperty>
  <owl:DatatypeProperty rdf:about="http://example.org/onto/prop/yandex_organizationmanager_user_ssh_key_expires_at">
    <rdfs:label>expires_at</rdfs:label>
    <rdfs:comment>Used for temporary keys, if empty the key doesn't expire</rdfs:comment>
    <rdfs:domain rdf:resource="http://example.org/onto/class/yandex_organizationmanager_user_ssh_key"/>
    <rdfs:range rdf:resource="http://www.w3.org/2001/XMLSchema#string"/>
  </owl:DatatypeProperty>
  <owl:DatatypeProperty rdf:about="http://example.org/onto/prop/yandex_organizationmanager_user_ssh_key_fingerprint">
    <rdfs:label>fingerprint</rdfs:label>
    <rdfs:comment>package: yandex.cloud.organizationmanager.v1
filename: yandex/cloud/organizationmanager/v1/user_ssh_key.proto</rdfs:comment>
    <rdfs:domain rdf:resource="http://example.org/onto/class/yandex_organizationmanager_user_ssh_key"/>
    <rdfs:range rdf:resource="http://www.w3.org/2001/XMLSchema#string"/>
  </owl:DatatypeProperty>
  <owl:DatatypeProperty rdf:about="http://example.org/onto/prop/yandex_organizationmanager_user_ssh_key_id">
    <rdfs:label>id</rdfs:label>
    <rdfs:comment>package: yandex.cloud.organizationmanager.v1
filename: yandex/cloud/organizationmanager/v1/user_ssh_key_service.proto</rdfs:comment>
    <rdfs:domain rdf:resource="http://example.org/onto/class/yandex_organizationmanager_user_ssh_key"/>
    <rdfs:range rdf:resource="http://www.w3.org/2001/XMLSchema#string"/>
  </owl:DatatypeProperty>
  <owl:DatatypeProperty rdf:about="http://example.org/onto/prop/yandex_organizationmanager_user_ssh_key_name">
    <rdfs:label>name</rdfs:label>
    <rdfs:comment>package: yandex.cloud.organizationmanager.v1
filename: yandex/cloud/organizationmanager/v1/user_ssh_key.proto</rdfs:comment>
    <rdfs:domain rdf:resource="http://example.org/onto/class/yandex_organizationmanager_user_ssh_key"/>
    <rdfs:range rdf:resource="http://www.w3.org/2001/XMLSchema#string"/>
  </owl:DatatypeProperty>
  <owl:DatatypeProperty rdf:about="http://example.org/onto/prop/yandex_organizationmanager_user_ssh_key_organization_id">
    <rdfs:label>organization_id</rdfs:label>
    <rdfs:comment>package: yandex.cloud.organizationmanager.v1
filename: yandex/cloud/organizationmanager/v1/user_ssh_key.proto</rdfs:comment>
    <rdfs:domain rdf:resource="http://example.org/onto/class/yandex_organizationmanager_user_ssh_key"/>
    <rdfs:range rdf:resource="http://www.w3.org/2001/XMLSchema#string"/>
  </owl:DatatypeProperty>
  <owl:DatatypeProperty rdf:about="http://example.org/onto/prop/yandex_organizationmanager_user_ssh_key_subject_id">
    <rdfs:label>subject_id</rdfs:label>
    <rdfs:comment>package: yandex.cloud.organizationmanager.v1
filename: yandex/cloud/organizationmanager/v1/user_ssh_key.proto</rdfs:comment>
    <rdfs:domain rdf:resource="http://example.org/onto/class/yandex_organizationmanager_user_ssh_key"/>
    <rdfs:range rdf:resource="http://www.w3.org/2001/XMLSchema#string"/>
  </owl:DatatypeProperty>
  <owl:DatatypeProperty rdf:about="http://example.org/onto/prop/yandex_organizationmanager_user_ssh_key_user_ssh_key_id">
    <rdfs:label>user_ssh_key_id</rdfs:label>
    <rdfs:comment>package: yandex.cloud.organizationmanager.v1
filename: yandex/cloud/organizationmanager/v1/user_ssh_key_service.proto</rdfs:comment>
    <rdfs:domain rdf:resource="http://example.org/onto/class/yandex_organizationmanager_user_ssh_key"/>
    <rdfs:range rdf:resource="http://www.w3.org/2001/XMLSchema#string"/>
  </owl:DatatypeProperty>
  <owl:DatatypeProperty rdf:about="http://example.org/onto/prop/yandex_organizationmanager_user_ssh_key_create">
    <rdfs:label>create</rdfs:label>
    <rdfs:comment>A string that can be [parsed as a duration](https://pkg.go.dev/time#ParseDuration) consisting of numbers and unit suffixes, such as "30s" or "2h45m". Valid time units are "s" (seconds), "m" (minutes), "h" (hours).</rdfs:comment>
    <rdfs:domain rdf:resource="http://example.org/onto/class/yandex_organizationmanager_user_ssh_key"/>
    <rdfs:range rdf:resource="http://www.w3.org/2001/XMLSchema#string"/>
  </owl:DatatypeProperty>
  <owl:DatatypeProperty rdf:about="http://example.org/onto/prop/yandex_organizationmanager_user_ssh_key_delete">
    <rdfs:label>delete</rdfs:label>
    <rdfs:comment>A string that can be [parsed as a duration](https://pkg.go.dev/time#ParseDuration) consisting of numbers and unit suffixes, such as "30s" or "2h45m". Valid time units are "s" (seconds), "m" (minutes), "h" (hours). Setting a timeout for a Delete operation is only applicable if changes are saved into state before the destroy operation occurs.</rdfs:comment>
    <rdfs:domain rdf:resource="http://example.org/onto/class/yandex_organizationmanager_user_ssh_key"/>
    <rdfs:range rdf:resource="http://www.w3.org/2001/XMLSchema#string"/>
  </owl:DatatypeProperty>
  <owl:DatatypeProperty rdf:about="http://example.org/onto/prop/yandex_organizationmanager_user_ssh_key_read">
    <rdfs:label>read</rdfs:label>
    <rdfs:comment>A string that can be [parsed as a duration](https://pkg.go.dev/time#ParseDuration) consisting of numbers and unit suffixes, such as "30s" or "2h45m". Valid time units are "s" (seconds), "m" (minutes), "h" (hours). Read operations occur during any refresh or planning operation when refresh is enabled.</rdfs:comment>
    <rdfs:domain rdf:resource="http://example.org/onto/class/yandex_organizationmanager_user_ssh_key"/>
    <rdfs:range rdf:resource="http://www.w3.org/2001/XMLSchema#string"/>
  </owl:DatatypeProperty>
  <owl:DatatypeProperty rdf:about="http://example.org/onto/prop/yandex_organizationmanager_user_ssh_key_update">
    <rdfs:label>update</rdfs:label>
    <rdfs:comment>A string that can be [parsed as a duration](https://pkg.go.dev/time#ParseDuration) consisting of numbers and unit suffixes, such as "30s" or "2h45m". Valid time units are "s" (seconds), "m" (minutes), "h" (hours).</rdfs:comment>
    <rdfs:domain rdf:resource="http://example.org/onto/class/yandex_organizationmanager_user_ssh_key"/>
    <rdfs:range rdf:resource="http://www.w3.org/2001/XMLSchema#string"/>
  </owl:DatatypeProperty>
</rdf:RDF>
