<?xml version="1.0" encoding="UTF-8"?>
<rdf:RDF
  xmlns:rdf="http://www.w3.org/1999/02/22-rdf-syntax-ns#"
  xmlns:rdfs="http://www.w3.org/2000/01/rdf-schema#"
  xmlns:owl="http://www.w3.org/2002/07/owl#"
  xmlns:xsd="http://www.w3.org/2001/XMLSchema#"
  xml:base="http://example.org/onto/">
  <owl:Class rdf:about="http://example.org/onto/class/yandex_mdb_kafka_cluster">
    <rdfs:label>yandex_mdb_kafka_cluster</rdfs:label>
    <rdfs:comment>Manages a Kafka cluster within the Yandex Cloud. For more information, see [the official documentation](https://yandex.cloud/docs/managed-kafka/concepts).

~> Historically, `topic` blocks of the `yandex_mdb_kafka_cluster` resource were used to manage topics of the Kafka cluster. However, this approach has a number of disadvantages. In particular, when adding and removing topics from the tf recipe, terraform generates a diff that misleads the user about the planned changes. Also, this approach turned out to be inconvenient when managing topics through the Kafka Admin API. Therefore, topic management through a separate resource type `yandex_mdb_kafka_topic` was implemented and is now recommended.</rdfs:comment>
  </owl:Class>
  <owl:DatatypeProperty rdf:about="http://example.org/onto/prop/yandex_mdb_kafka_cluster_created_at">
    <rdfs:label>created_at</rdfs:label>
    <rdfs:comment>The creation timestamp of the resource.</rdfs:comment>
    <rdfs:domain rdf:resource="http://example.org/onto/class/yandex_mdb_kafka_cluster"/>
    <rdfs:range rdf:resource="http://www.w3.org/2001/XMLSchema#string"/>
  </owl:DatatypeProperty>
  <owl:DatatypeProperty rdf:about="http://example.org/onto/prop/yandex_mdb_kafka_cluster_deletion_protection">
    <rdfs:label>deletion_protection</rdfs:label>
    <rdfs:comment>The `true` value means that resource is protected from accidental deletion.</rdfs:comment>
    <rdfs:domain rdf:resource="http://example.org/onto/class/yandex_mdb_kafka_cluster"/>
    <rdfs:range rdf:resource="http://www.w3.org/2001/XMLSchema#string"/>
  </owl:DatatypeProperty>
  <owl:DatatypeProperty rdf:about="http://example.org/onto/prop/yandex_mdb_kafka_cluster_description">
    <rdfs:label>description</rdfs:label>
    <rdfs:comment>The resource description.</rdfs:comment>
    <rdfs:domain rdf:resource="http://example.org/onto/class/yandex_mdb_kafka_cluster"/>
    <rdfs:range rdf:resource="http://www.w3.org/2001/XMLSchema#string"/>
  </owl:DatatypeProperty>
  <owl:DatatypeProperty rdf:about="http://example.org/onto/prop/yandex_mdb_kafka_cluster_environment">
    <rdfs:label>environment</rdfs:label>
    <rdfs:comment>Deployment environment of the Kafka cluster. Can be either `PRESTABLE` or `PRODUCTION`. The default is `PRODUCTION`.</rdfs:comment>
    <rdfs:domain rdf:resource="http://example.org/onto/class/yandex_mdb_kafka_cluster"/>
    <rdfs:range rdf:resource="http://www.w3.org/2001/XMLSchema#string"/>
  </owl:DatatypeProperty>
  <owl:DatatypeProperty rdf:about="http://example.org/onto/prop/yandex_mdb_kafka_cluster_folder_id">
    <rdfs:label>folder_id</rdfs:label>
    <rdfs:comment>The folder identifier that resource belongs to. If it is not provided, the default provider `folder-id` is used.</rdfs:comment>
    <rdfs:domain rdf:resource="http://example.org/onto/class/yandex_mdb_kafka_cluster"/>
    <rdfs:range rdf:resource="http://www.w3.org/2001/XMLSchema#string"/>
  </owl:DatatypeProperty>
  <owl:DatatypeProperty rdf:about="http://example.org/onto/prop/yandex_mdb_kafka_cluster_health">
    <rdfs:label>health</rdfs:label>
    <rdfs:comment>Aggregated health of the cluster. Can be either `ALIVE`, `DEGRADED`, `DEAD` or `HEALTH_UNKNOWN`. For more information see `health` field of JSON representation in [the official documentation](https://yandex.cloud/docs/managed-kafka/api-ref/Cluster/).</rdfs:comment>
    <rdfs:domain rdf:resource="http://example.org/onto/class/yandex_mdb_kafka_cluster"/>
    <rdfs:range rdf:resource="http://www.w3.org/2001/XMLSchema#string"/>
  </owl:DatatypeProperty>
  <owl:DatatypeProperty rdf:about="http://example.org/onto/prop/yandex_mdb_kafka_cluster_host">
    <rdfs:label>host</rdfs:label>
    <rdfs:comment>A host of the Kafka cluster.</rdfs:comment>
    <rdfs:domain rdf:resource="http://example.org/onto/class/yandex_mdb_kafka_cluster"/>
    <rdfs:range rdf:resource="http://www.w3.org/2001/XMLSchema#string"/>
  </owl:DatatypeProperty>
  <owl:DatatypeProperty rdf:about="http://example.org/onto/prop/yandex_mdb_kafka_cluster_host_group_ids">
    <rdfs:label>host_group_ids</rdfs:label>
    <rdfs:comment>A list of IDs of the host groups to place VMs of the cluster on.</rdfs:comment>
    <rdfs:domain rdf:resource="http://example.org/onto/class/yandex_mdb_kafka_cluster"/>
    <rdfs:range rdf:resource="http://www.w3.org/2001/XMLSchema#string"/>
  </owl:DatatypeProperty>
  <owl:DatatypeProperty rdf:about="http://example.org/onto/prop/yandex_mdb_kafka_cluster_id">
    <rdfs:label>id</rdfs:label>
    <rdfs:domain rdf:resource="http://example.org/onto/class/yandex_mdb_kafka_cluster"/>
    <rdfs:range rdf:resource="http://www.w3.org/2001/XMLSchema#string"/>
  </owl:DatatypeProperty>
  <owl:DatatypeProperty rdf:about="http://example.org/onto/prop/yandex_mdb_kafka_cluster_labels">
    <rdfs:label>labels</rdfs:label>
    <rdfs:comment>A set of key/value label pairs which assigned to resource.</rdfs:comment>
    <rdfs:domain rdf:resource="http://example.org/onto/class/yandex_mdb_kafka_cluster"/>
    <rdfs:range rdf:resource="http://www.w3.org/2001/XMLSchema#string"/>
  </owl:DatatypeProperty>
  <owl:DatatypeProperty rdf:about="http://example.org/onto/prop/yandex_mdb_kafka_cluster_name">
    <rdfs:label>name</rdfs:label>
    <rdfs:comment>The resource name.</rdfs:comment>
    <rdfs:domain rdf:resource="http://example.org/onto/class/yandex_mdb_kafka_cluster"/>
    <rdfs:range rdf:resource="http://www.w3.org/2001/XMLSchema#string"/>
  </owl:DatatypeProperty>
  <owl:DatatypeProperty rdf:about="http://example.org/onto/prop/yandex_mdb_kafka_cluster_network_id">
    <rdfs:label>network_id</rdfs:label>
    <rdfs:comment>The `VPC Network ID` of subnets which resource attached to.</rdfs:comment>
    <rdfs:domain rdf:resource="http://example.org/onto/class/yandex_mdb_kafka_cluster"/>
    <rdfs:range rdf:resource="http://www.w3.org/2001/XMLSchema#string"/>
  </owl:DatatypeProperty>
  <owl:DatatypeProperty rdf:about="http://example.org/onto/prop/yandex_mdb_kafka_cluster_security_group_ids">
    <rdfs:label>security_group_ids</rdfs:label>
    <rdfs:comment>The list of security groups applied to resource or their components.</rdfs:comment>
    <rdfs:domain rdf:resource="http://example.org/onto/class/yandex_mdb_kafka_cluster"/>
    <rdfs:range rdf:resource="http://www.w3.org/2001/XMLSchema#string"/>
  </owl:DatatypeProperty>
  <owl:DatatypeProperty rdf:about="http://example.org/onto/prop/yandex_mdb_kafka_cluster_status">
    <rdfs:label>status</rdfs:label>
    <rdfs:comment>Status of the cluster. Can be either `CREATING`, `STARTING`, `RUNNING`, `UPDATING`, `STOPPING`, `STOPPED`, `ERROR` or `STATUS_UNKNOWN`. For more information see `status` field of JSON representation in [the official documentation](https://yandex.cloud/docs/managed-kafka/api-ref/Cluster/).</rdfs:comment>
    <rdfs:domain rdf:resource="http://example.org/onto/class/yandex_mdb_kafka_cluster"/>
    <rdfs:range rdf:resource="http://www.w3.org/2001/XMLSchema#string"/>
  </owl:DatatypeProperty>
  <owl:DatatypeProperty rdf:about="http://example.org/onto/prop/yandex_mdb_kafka_cluster_subnet_ids">
    <rdfs:label>subnet_ids</rdfs:label>
    <rdfs:comment>The list of VPC subnets identifiers which resource is attached.</rdfs:comment>
    <rdfs:domain rdf:resource="http://example.org/onto/class/yandex_mdb_kafka_cluster"/>
    <rdfs:range rdf:resource="http://www.w3.org/2001/XMLSchema#string"/>
  </owl:DatatypeProperty>
  <owl:DatatypeProperty rdf:about="http://example.org/onto/prop/yandex_mdb_kafka_cluster_assign_public_ip">
    <rdfs:label>assign_public_ip</rdfs:label>
    <rdfs:comment>Determines whether each broker will be assigned a public IP address. The default is `false`.</rdfs:comment>
    <rdfs:domain rdf:resource="http://example.org/onto/class/yandex_mdb_kafka_cluster"/>
    <rdfs:range rdf:resource="http://www.w3.org/2001/XMLSchema#string"/>
  </owl:DatatypeProperty>
  <owl:DatatypeProperty rdf:about="http://example.org/onto/prop/yandex_mdb_kafka_cluster_brokers_count">
    <rdfs:label>brokers_count</rdfs:label>
    <rdfs:comment>Count of brokers per availability zone. The default is `1`.</rdfs:comment>
    <rdfs:domain rdf:resource="http://example.org/onto/class/yandex_mdb_kafka_cluster"/>
    <rdfs:range rdf:resource="http://www.w3.org/2001/XMLSchema#string"/>
  </owl:DatatypeProperty>
  <owl:DatatypeProperty rdf:about="http://example.org/onto/prop/yandex_mdb_kafka_cluster_schema_registry">
    <rdfs:label>schema_registry</rdfs:label>
    <rdfs:comment>Enables managed schema registry on cluster. The default is `false`.</rdfs:comment>
    <rdfs:domain rdf:resource="http://example.org/onto/class/yandex_mdb_kafka_cluster"/>
    <rdfs:range rdf:resource="http://www.w3.org/2001/XMLSchema#string"/>
  </owl:DatatypeProperty>
  <owl:DatatypeProperty rdf:about="http://example.org/onto/prop/yandex_mdb_kafka_cluster_unmanaged_topics">
    <rdfs:label>unmanaged_topics</rdfs:label>
    <rdfs:domain rdf:resource="http://example.org/onto/class/yandex_mdb_kafka_cluster"/>
    <rdfs:range rdf:resource="http://www.w3.org/2001/XMLSchema#string"/>
  </owl:DatatypeProperty>
  <owl:DatatypeProperty rdf:about="http://example.org/onto/prop/yandex_mdb_kafka_cluster_version">
    <rdfs:label>version</rdfs:label>
    <rdfs:comment>Version of the Kafka server software.</rdfs:comment>
    <rdfs:domain rdf:resource="http://example.org/onto/class/yandex_mdb_kafka_cluster"/>
    <rdfs:range rdf:resource="http://www.w3.org/2001/XMLSchema#string"/>
  </owl:DatatypeProperty>
  <owl:DatatypeProperty rdf:about="http://example.org/onto/prop/yandex_mdb_kafka_cluster_zones">
    <rdfs:label>zones</rdfs:label>
    <rdfs:comment>List of availability zones.</rdfs:comment>
    <rdfs:domain rdf:resource="http://example.org/onto/class/yandex_mdb_kafka_cluster"/>
    <rdfs:range rdf:resource="http://www.w3.org/2001/XMLSchema#string"/>
  </owl:DatatypeProperty>
  <owl:DatatypeProperty rdf:about="http://example.org/onto/prop/yandex_mdb_kafka_cluster_data_transfer">
    <rdfs:label>data_transfer</rdfs:label>
    <rdfs:comment>Allow access for [DataTransfer](https://yandex.cloud/services/data-transfer).</rdfs:comment>
    <rdfs:domain rdf:resource="http://example.org/onto/class/yandex_mdb_kafka_cluster"/>
    <rdfs:range rdf:resource="http://www.w3.org/2001/XMLSchema#string"/>
  </owl:DatatypeProperty>
  <owl:DatatypeProperty rdf:about="http://example.org/onto/prop/yandex_mdb_kafka_cluster_disk_size_limit">
    <rdfs:label>disk_size_limit</rdfs:label>
    <rdfs:comment>Maximum possible size of disk in bytes.</rdfs:comment>
    <rdfs:domain rdf:resource="http://example.org/onto/class/yandex_mdb_kafka_cluster"/>
    <rdfs:range rdf:resource="http://www.w3.org/2001/XMLSchema#string"/>
  </owl:DatatypeProperty>
  <owl:DatatypeProperty rdf:about="http://example.org/onto/prop/yandex_mdb_kafka_cluster_emergency_usage_threshold">
    <rdfs:label>emergency_usage_threshold</rdfs:label>
    <rdfs:comment>Percent of disk utilization. Disk will autoscale immediately, if this threshold reached. Value is between 0 and 100. Default value is 0 (autoscaling disabled). Must be not less then 'planned_usage_threshold' value.</rdfs:comment>
    <rdfs:domain rdf:resource="http://example.org/onto/class/yandex_mdb_kafka_cluster"/>
    <rdfs:range rdf:resource="http://www.w3.org/2001/XMLSchema#string"/>
  </owl:DatatypeProperty>
  <owl:DatatypeProperty rdf:about="http://example.org/onto/prop/yandex_mdb_kafka_cluster_planned_usage_threshold">
    <rdfs:label>planned_usage_threshold</rdfs:label>
    <rdfs:comment>Percent of disk utilization. During maintenance disk will autoscale, if this threshold reached. Value is between 0 and 100. Default value is 0 (autoscaling disabled).</rdfs:comment>
    <rdfs:domain rdf:resource="http://example.org/onto/class/yandex_mdb_kafka_cluster"/>
    <rdfs:range rdf:resource="http://www.w3.org/2001/XMLSchema#string"/>
  </owl:DatatypeProperty>
  <owl:DatatypeProperty rdf:about="http://example.org/onto/prop/yandex_mdb_kafka_cluster_auto_create_topics_enable">
    <rdfs:label>auto_create_topics_enable</rdfs:label>
    <rdfs:comment>Enable auto creation of topic on the server.</rdfs:comment>
    <rdfs:domain rdf:resource="http://example.org/onto/class/yandex_mdb_kafka_cluster"/>
    <rdfs:range rdf:resource="http://www.w3.org/2001/XMLSchema#string"/>
  </owl:DatatypeProperty>
  <owl:DatatypeProperty rdf:about="http://example.org/onto/prop/yandex_mdb_kafka_cluster_compression_type">
    <rdfs:label>compression_type</rdfs:label>
    <rdfs:comment>Compression type of kafka topics.</rdfs:comment>
    <rdfs:domain rdf:resource="http://example.org/onto/class/yandex_mdb_kafka_cluster"/>
    <rdfs:range rdf:resource="http://www.w3.org/2001/XMLSchema#string"/>
  </owl:DatatypeProperty>
  <owl:DatatypeProperty rdf:about="http://example.org/onto/prop/yandex_mdb_kafka_cluster_default_replication_factor">
    <rdfs:label>default_replication_factor</rdfs:label>
    <rdfs:comment>The replication factor for automatically created topics, and for topics created with -1 as the replication factor.</rdfs:comment>
    <rdfs:domain rdf:resource="http://example.org/onto/class/yandex_mdb_kafka_cluster"/>
    <rdfs:range rdf:resource="http://www.w3.org/2001/XMLSchema#string"/>
  </owl:DatatypeProperty>
  <owl:DatatypeProperty rdf:about="http://example.org/onto/prop/yandex_mdb_kafka_cluster_log_flush_interval_messages">
    <rdfs:label>log_flush_interval_messages</rdfs:label>
    <rdfs:comment>The number of messages accumulated on a log partition before messages are flushed to disk.</rdfs:comment>
    <rdfs:domain rdf:resource="http://example.org/onto/class/yandex_mdb_kafka_cluster"/>
    <rdfs:range rdf:resource="http://www.w3.org/2001/XMLSchema#string"/>
  </owl:DatatypeProperty>
  <owl:DatatypeProperty rdf:about="http://example.org/onto/prop/yandex_mdb_kafka_cluster_log_flush_interval_ms">
    <rdfs:label>log_flush_interval_ms</rdfs:label>
    <rdfs:comment>The maximum time in ms that a message in any topic is kept in memory before flushed to disk. If not set, the value in log.flush.scheduler.interval.ms is used.</rdfs:comment>
    <rdfs:domain rdf:resource="http://example.org/onto/class/yandex_mdb_kafka_cluster"/>
    <rdfs:range rdf:resource="http://www.w3.org/2001/XMLSchema#string"/>
  </owl:DatatypeProperty>
  <owl:DatatypeProperty rdf:about="http://example.org/onto/prop/yandex_mdb_kafka_cluster_log_flush_scheduler_interval_ms">
    <rdfs:label>log_flush_scheduler_interval_ms</rdfs:label>
    <rdfs:comment>The frequency in ms that the log flusher checks whether any log needs to be flushed to disk.</rdfs:comment>
    <rdfs:domain rdf:resource="http://example.org/onto/class/yandex_mdb_kafka_cluster"/>
    <rdfs:range rdf:resource="http://www.w3.org/2001/XMLSchema#string"/>
  </owl:DatatypeProperty>
  <owl:DatatypeProperty rdf:about="http://example.org/onto/prop/yandex_mdb_kafka_cluster_log_preallocate">
    <rdfs:label>log_preallocate</rdfs:label>
    <rdfs:comment>Should pre allocate file when create new segment?</rdfs:comment>
    <rdfs:domain rdf:resource="http://example.org/onto/class/yandex_mdb_kafka_cluster"/>
    <rdfs:range rdf:resource="http://www.w3.org/2001/XMLSchema#string"/>
  </owl:DatatypeProperty>
  <owl:DatatypeProperty rdf:about="http://example.org/onto/prop/yandex_mdb_kafka_cluster_log_retention_bytes">
    <rdfs:label>log_retention_bytes</rdfs:label>
    <rdfs:comment>The maximum size of the log before deleting it.</rdfs:comment>
    <rdfs:domain rdf:resource="http://example.org/onto/class/yandex_mdb_kafka_cluster"/>
    <rdfs:range rdf:resource="http://www.w3.org/2001/XMLSchema#string"/>
  </owl:DatatypeProperty>
  <owl:DatatypeProperty rdf:about="http://example.org/onto/prop/yandex_mdb_kafka_cluster_log_retention_hours">
    <rdfs:label>log_retention_hours</rdfs:label>
    <rdfs:comment>The number of hours to keep a log file before deleting it (in hours), tertiary to log.retention.ms property.</rdfs:comment>
    <rdfs:domain rdf:resource="http://example.org/onto/class/yandex_mdb_kafka_cluster"/>
    <rdfs:range rdf:resource="http://www.w3.org/2001/XMLSchema#string"/>
  </owl:DatatypeProperty>
  <owl:DatatypeProperty rdf:about="http://example.org/onto/prop/yandex_mdb_kafka_cluster_log_retention_minutes">
    <rdfs:label>log_retention_minutes</rdfs:label>
    <rdfs:comment>The number of minutes to keep a log file before deleting it (in minutes), secondary to log.retention.ms property. If not set, the value in log.retention.hours is used.</rdfs:comment>
    <rdfs:domain rdf:resource="http://example.org/onto/class/yandex_mdb_kafka_cluster"/>
    <rdfs:range rdf:resource="http://www.w3.org/2001/XMLSchema#string"/>
  </owl:DatatypeProperty>
  <owl:DatatypeProperty rdf:about="http://example.org/onto/prop/yandex_mdb_kafka_cluster_log_retention_ms">
    <rdfs:label>log_retention_ms</rdfs:label>
    <rdfs:comment>The number of milliseconds to keep a log file before deleting it (in milliseconds), If not set, the value in log.retention.minutes is used. If set to -1, no time limit is applied.</rdfs:comment>
    <rdfs:domain rdf:resource="http://example.org/onto/class/yandex_mdb_kafka_cluster"/>
    <rdfs:range rdf:resource="http://www.w3.org/2001/XMLSchema#string"/>
  </owl:DatatypeProperty>
  <owl:DatatypeProperty rdf:about="http://example.org/onto/prop/yandex_mdb_kafka_cluster_log_segment_bytes">
    <rdfs:label>log_segment_bytes</rdfs:label>
    <rdfs:comment>The maximum size of a single log file.</rdfs:comment>
    <rdfs:domain rdf:resource="http://example.org/onto/class/yandex_mdb_kafka_cluster"/>
    <rdfs:range rdf:resource="http://www.w3.org/2001/XMLSchema#string"/>
  </owl:DatatypeProperty>
  <owl:DatatypeProperty rdf:about="http://example.org/onto/prop/yandex_mdb_kafka_cluster_message_max_bytes">
    <rdfs:label>message_max_bytes</rdfs:label>
    <rdfs:comment>The largest record batch size allowed by Kafka (after compression if compression is enabled).</rdfs:comment>
    <rdfs:domain rdf:resource="http://example.org/onto/class/yandex_mdb_kafka_cluster"/>
    <rdfs:range rdf:resource="http://www.w3.org/2001/XMLSchema#string"/>
  </owl:DatatypeProperty>
  <owl:DatatypeProperty rdf:about="http://example.org/onto/prop/yandex_mdb_kafka_cluster_num_partitions">
    <rdfs:label>num_partitions</rdfs:label>
    <rdfs:comment>The default number of log partitions per topic.</rdfs:comment>
    <rdfs:domain rdf:resource="http://example.org/onto/class/yandex_mdb_kafka_cluster"/>
    <rdfs:range rdf:resource="http://www.w3.org/2001/XMLSchema#string"/>
  </owl:DatatypeProperty>
  <owl:DatatypeProperty rdf:about="http://example.org/onto/prop/yandex_mdb_kafka_cluster_offsets_retention_minutes">
    <rdfs:label>offsets_retention_minutes</rdfs:label>
    <rdfs:comment>For subscribed consumers, committed offset of a specific partition will be expired and discarded after this period of time.</rdfs:comment>
    <rdfs:domain rdf:resource="http://example.org/onto/class/yandex_mdb_kafka_cluster"/>
    <rdfs:range rdf:resource="http://www.w3.org/2001/XMLSchema#string"/>
  </owl:DatatypeProperty>
  <owl:DatatypeProperty rdf:about="http://example.org/onto/prop/yandex_mdb_kafka_cluster_replica_fetch_max_bytes">
    <rdfs:label>replica_fetch_max_bytes</rdfs:label>
    <rdfs:comment>The number of bytes of messages to attempt to fetch for each partition.</rdfs:comment>
    <rdfs:domain rdf:resource="http://example.org/onto/class/yandex_mdb_kafka_cluster"/>
    <rdfs:range rdf:resource="http://www.w3.org/2001/XMLSchema#string"/>
  </owl:DatatypeProperty>
  <owl:DatatypeProperty rdf:about="http://example.org/onto/prop/yandex_mdb_kafka_cluster_sasl_enabled_mechanisms">
    <rdfs:label>sasl_enabled_mechanisms</rdfs:label>
    <rdfs:comment>The list of SASL mechanisms enabled in the Kafka server.</rdfs:comment>
    <rdfs:domain rdf:resource="http://example.org/onto/class/yandex_mdb_kafka_cluster"/>
    <rdfs:range rdf:resource="http://www.w3.org/2001/XMLSchema#string"/>
  </owl:DatatypeProperty>
  <owl:DatatypeProperty rdf:about="http://example.org/onto/prop/yandex_mdb_kafka_cluster_socket_receive_buffer_bytes">
    <rdfs:label>socket_receive_buffer_bytes</rdfs:label>
    <rdfs:comment>The SO_RCVBUF buffer of the socket server sockets. If the value is -1, the OS default will be used.</rdfs:comment>
    <rdfs:domain rdf:resource="http://example.org/onto/class/yandex_mdb_kafka_cluster"/>
    <rdfs:range rdf:resource="http://www.w3.org/2001/XMLSchema#string"/>
  </owl:DatatypeProperty>
  <owl:DatatypeProperty rdf:about="http://example.org/onto/prop/yandex_mdb_kafka_cluster_socket_send_buffer_bytes">
    <rdfs:label>socket_send_buffer_bytes</rdfs:label>
    <rdfs:comment>The SO_SNDBUF buffer of the socket server sockets. If the value is -1, the OS default will be used.</rdfs:comment>
    <rdfs:domain rdf:resource="http://example.org/onto/class/yandex_mdb_kafka_cluster"/>
    <rdfs:range rdf:resource="http://www.w3.org/2001/XMLSchema#string"/>
  </owl:DatatypeProperty>
  <owl:DatatypeProperty rdf:about="http://example.org/onto/prop/yandex_mdb_kafka_cluster_ssl_cipher_suites">
    <rdfs:label>ssl_cipher_suites</rdfs:label>
    <rdfs:comment>A list of cipher suites.</rdfs:comment>
    <rdfs:domain rdf:resource="http://example.org/onto/class/yandex_mdb_kafka_cluster"/>
    <rdfs:range rdf:resource="http://www.w3.org/2001/XMLSchema#string"/>
  </owl:DatatypeProperty>
  <owl:DatatypeProperty rdf:about="http://example.org/onto/prop/yandex_mdb_kafka_cluster_disk_size">
    <rdfs:label>disk_size</rdfs:label>
    <rdfs:comment>Volume of the storage available to a Kafka host, in gigabytes.</rdfs:comment>
    <rdfs:domain rdf:resource="http://example.org/onto/class/yandex_mdb_kafka_cluster"/>
    <rdfs:range rdf:resource="http://www.w3.org/2001/XMLSchema#string"/>
  </owl:DatatypeProperty>
  <owl:DatatypeProperty rdf:about="http://example.org/onto/prop/yandex_mdb_kafka_cluster_disk_type_id">
    <rdfs:label>disk_type_id</rdfs:label>
    <rdfs:comment>Type of the storage of Kafka hosts. For more information see [the official documentation](https://yandex.cloud/docs/managed-kafka/concepts/storage).</rdfs:comment>
    <rdfs:domain rdf:resource="http://example.org/onto/class/yandex_mdb_kafka_cluster"/>
    <rdfs:range rdf:resource="http://www.w3.org/2001/XMLSchema#string"/>
  </owl:DatatypeProperty>
  <owl:DatatypeProperty rdf:about="http://example.org/onto/prop/yandex_mdb_kafka_cluster_resource_preset_id">
    <rdfs:label>resource_preset_id</rdfs:label>
    <rdfs:comment>The ID of the preset for computational resources available to a Kafka host (CPU, memory etc.). For more information, see [the official documentation](https://yandex.cloud/docs/managed-kafka/concepts).</rdfs:comment>
    <rdfs:domain rdf:resource="http://example.org/onto/class/yandex_mdb_kafka_cluster"/>
    <rdfs:range rdf:resource="http://www.w3.org/2001/XMLSchema#string"/>
  </owl:DatatypeProperty>
  <owl:DatatypeProperty rdf:about="http://example.org/onto/prop/yandex_mdb_kafka_cluster_enabled">
    <rdfs:label>enabled</rdfs:label>
    <rdfs:comment>Enables KAFKA UI on cluster. The default is `false`.</rdfs:comment>
    <rdfs:domain rdf:resource="http://example.org/onto/class/yandex_mdb_kafka_cluster"/>
    <rdfs:range rdf:resource="http://www.w3.org/2001/XMLSchema#string"/>
  </owl:DatatypeProperty>
  <owl:DatatypeProperty rdf:about="http://example.org/onto/prop/yandex_mdb_kafka_cluster_disk_size">
    <rdfs:label>disk_size</rdfs:label>
    <rdfs:comment>Volume of the storage available to a KRaft-controller host, in gigabytes.</rdfs:comment>
    <rdfs:domain rdf:resource="http://example.org/onto/class/yandex_mdb_kafka_cluster"/>
    <rdfs:range rdf:resource="http://www.w3.org/2001/XMLSchema#string"/>
  </owl:DatatypeProperty>
  <owl:DatatypeProperty rdf:about="http://example.org/onto/prop/yandex_mdb_kafka_cluster_disk_type_id">
    <rdfs:label>disk_type_id</rdfs:label>
    <rdfs:comment>Type of the storage of KRaft-controller hosts. For more information see [the official documentation](https://yandex.cloud/docs/managed-kafka/concepts/storage).</rdfs:comment>
    <rdfs:domain rdf:resource="http://example.org/onto/class/yandex_mdb_kafka_cluster"/>
    <rdfs:range rdf:resource="http://www.w3.org/2001/XMLSchema#string"/>
  </owl:DatatypeProperty>
  <owl:DatatypeProperty rdf:about="http://example.org/onto/prop/yandex_mdb_kafka_cluster_resource_preset_id">
    <rdfs:label>resource_preset_id</rdfs:label>
    <rdfs:comment>The ID of the preset for computational resources available to a KRaft-controller host (CPU, memory etc.). For more information, see [the official documentation](https://yandex.cloud/docs/managed-kafka/concepts).</rdfs:comment>
    <rdfs:domain rdf:resource="http://example.org/onto/class/yandex_mdb_kafka_cluster"/>
    <rdfs:range rdf:resource="http://www.w3.org/2001/XMLSchema#string"/>
  </owl:DatatypeProperty>
  <owl:DatatypeProperty rdf:about="http://example.org/onto/prop/yandex_mdb_kafka_cluster_enabled">
    <rdfs:label>enabled</rdfs:label>
    <rdfs:comment>Enables REST API on cluster. The default is `false`.</rdfs:comment>
    <rdfs:domain rdf:resource="http://example.org/onto/class/yandex_mdb_kafka_cluster"/>
    <rdfs:range rdf:resource="http://www.w3.org/2001/XMLSchema#string"/>
  </owl:DatatypeProperty>
  <owl:DatatypeProperty rdf:about="http://example.org/onto/prop/yandex_mdb_kafka_cluster_disk_size">
    <rdfs:label>disk_size</rdfs:label>
    <rdfs:comment>Volume of the storage available to a ZooKeeper host, in gigabytes.</rdfs:comment>
    <rdfs:domain rdf:resource="http://example.org/onto/class/yandex_mdb_kafka_cluster"/>
    <rdfs:range rdf:resource="http://www.w3.org/2001/XMLSchema#string"/>
  </owl:DatatypeProperty>
  <owl:DatatypeProperty rdf:about="http://example.org/onto/prop/yandex_mdb_kafka_cluster_disk_type_id">
    <rdfs:label>disk_type_id</rdfs:label>
    <rdfs:comment>Type of the storage of ZooKeeper hosts. For more information see [the official documentation](https://yandex.cloud/docs/managed-kafka/concepts/storage).</rdfs:comment>
    <rdfs:domain rdf:resource="http://example.org/onto/class/yandex_mdb_kafka_cluster"/>
    <rdfs:range rdf:resource="http://www.w3.org/2001/XMLSchema#string"/>
  </owl:DatatypeProperty>
  <owl:DatatypeProperty rdf:about="http://example.org/onto/prop/yandex_mdb_kafka_cluster_resource_preset_id">
    <rdfs:label>resource_preset_id</rdfs:label>
    <rdfs:comment>The ID of the preset for computational resources available to a ZooKeeper host (CPU, memory etc.). For more information, see [the official documentation](https://yandex.cloud/docs/managed-kafka/concepts).</rdfs:comment>
    <rdfs:domain rdf:resource="http://example.org/onto/class/yandex_mdb_kafka_cluster"/>
    <rdfs:range rdf:resource="http://www.w3.org/2001/XMLSchema#string"/>
  </owl:DatatypeProperty>
  <owl:DatatypeProperty rdf:about="http://example.org/onto/prop/yandex_mdb_kafka_cluster_day">
    <rdfs:label>day</rdfs:label>
    <rdfs:comment>Day of the week (in `DDD` format). Allowed values: `MON`, `TUE`, `WED`, `THU`, `FRI`, `SAT`, `SUN`.</rdfs:comment>
    <rdfs:domain rdf:resource="http://example.org/onto/class/yandex_mdb_kafka_cluster"/>
    <rdfs:range rdf:resource="http://www.w3.org/2001/XMLSchema#string"/>
  </owl:DatatypeProperty>
  <owl:DatatypeProperty rdf:about="http://example.org/onto/prop/yandex_mdb_kafka_cluster_hour">
    <rdfs:label>hour</rdfs:label>
    <rdfs:comment>Hour of the day in UTC (in `HH` format). Allowed value is between 1 and 24.</rdfs:comment>
    <rdfs:domain rdf:resource="http://example.org/onto/class/yandex_mdb_kafka_cluster"/>
    <rdfs:range rdf:resource="http://www.w3.org/2001/XMLSchema#string"/>
  </owl:DatatypeProperty>
  <owl:DatatypeProperty rdf:about="http://example.org/onto/prop/yandex_mdb_kafka_cluster_type">
    <rdfs:label>type</rdfs:label>
    <rdfs:comment>Type of maintenance window. Can be either `ANYTIME` or `WEEKLY`. A day and hour of window need to be specified with weekly window.</rdfs:comment>
    <rdfs:domain rdf:resource="http://example.org/onto/class/yandex_mdb_kafka_cluster"/>
    <rdfs:range rdf:resource="http://www.w3.org/2001/XMLSchema#string"/>
  </owl:DatatypeProperty>
  <owl:DatatypeProperty rdf:about="http://example.org/onto/prop/yandex_mdb_kafka_cluster_create">
    <rdfs:label>create</rdfs:label>
    <rdfs:domain rdf:resource="http://example.org/onto/class/yandex_mdb_kafka_cluster"/>
    <rdfs:range rdf:resource="http://www.w3.org/2001/XMLSchema#string"/>
  </owl:DatatypeProperty>
  <owl:DatatypeProperty rdf:about="http://example.org/onto/prop/yandex_mdb_kafka_cluster_delete">
    <rdfs:label>delete</rdfs:label>
    <rdfs:domain rdf:resource="http://example.org/onto/class/yandex_mdb_kafka_cluster"/>
    <rdfs:range rdf:resource="http://www.w3.org/2001/XMLSchema#string"/>
  </owl:DatatypeProperty>
  <owl:DatatypeProperty rdf:about="http://example.org/onto/prop/yandex_mdb_kafka_cluster_read">
    <rdfs:label>read</rdfs:label>
    <rdfs:domain rdf:resource="http://example.org/onto/class/yandex_mdb_kafka_cluster"/>
    <rdfs:range rdf:resource="http://www.w3.org/2001/XMLSchema#string"/>
  </owl:DatatypeProperty>
  <owl:DatatypeProperty rdf:about="http://example.org/onto/prop/yandex_mdb_kafka_cluster_update">
    <rdfs:label>update</rdfs:label>
    <rdfs:domain rdf:resource="http://example.org/onto/class/yandex_mdb_kafka_cluster"/>
    <rdfs:range rdf:resource="http://www.w3.org/2001/XMLSchema#string"/>
  </owl:DatatypeProperty>
  <owl:DatatypeProperty rdf:about="http://example.org/onto/prop/yandex_mdb_kafka_cluster_name">
    <rdfs:label>name</rdfs:label>
    <rdfs:comment>The name of the topic.</rdfs:comment>
    <rdfs:domain rdf:resource="http://example.org/onto/class/yandex_mdb_kafka_cluster"/>
    <rdfs:range rdf:resource="http://www.w3.org/2001/XMLSchema#string"/>
  </owl:DatatypeProperty>
  <owl:DatatypeProperty rdf:about="http://example.org/onto/prop/yandex_mdb_kafka_cluster_partitions">
    <rdfs:label>partitions</rdfs:label>
    <rdfs:comment>The number of the topic's partitions.</rdfs:comment>
    <rdfs:domain rdf:resource="http://example.org/onto/class/yandex_mdb_kafka_cluster"/>
    <rdfs:range rdf:resource="http://www.w3.org/2001/XMLSchema#string"/>
  </owl:DatatypeProperty>
  <owl:DatatypeProperty rdf:about="http://example.org/onto/prop/yandex_mdb_kafka_cluster_replication_factor">
    <rdfs:label>replication_factor</rdfs:label>
    <rdfs:comment>Amount of data copies (replicas) for the topic in the cluster.</rdfs:comment>
    <rdfs:domain rdf:resource="http://example.org/onto/class/yandex_mdb_kafka_cluster"/>
    <rdfs:range rdf:resource="http://www.w3.org/2001/XMLSchema#string"/>
  </owl:DatatypeProperty>
  <owl:DatatypeProperty rdf:about="http://example.org/onto/prop/yandex_mdb_kafka_cluster_cleanup_policy">
    <rdfs:label>cleanup_policy</rdfs:label>
    <rdfs:comment>Retention policy to use on log segments.</rdfs:comment>
    <rdfs:domain rdf:resource="http://example.org/onto/class/yandex_mdb_kafka_cluster"/>
    <rdfs:range rdf:resource="http://www.w3.org/2001/XMLSchema#string"/>
  </owl:DatatypeProperty>
  <owl:DatatypeProperty rdf:about="http://example.org/onto/prop/yandex_mdb_kafka_cluster_compression_type">
    <rdfs:label>compression_type</rdfs:label>
    <rdfs:comment>Compression type of kafka topic.</rdfs:comment>
    <rdfs:domain rdf:resource="http://example.org/onto/class/yandex_mdb_kafka_cluster"/>
    <rdfs:range rdf:resource="http://www.w3.org/2001/XMLSchema#string"/>
  </owl:DatatypeProperty>
  <owl:DatatypeProperty rdf:about="http://example.org/onto/prop/yandex_mdb_kafka_cluster_delete_retention_ms">
    <rdfs:label>delete_retention_ms</rdfs:label>
    <rdfs:comment>The amount of time to retain delete tombstone markers for log compacted topics.</rdfs:comment>
    <rdfs:domain rdf:resource="http://example.org/onto/class/yandex_mdb_kafka_cluster"/>
    <rdfs:range rdf:resource="http://www.w3.org/2001/XMLSchema#string"/>
  </owl:DatatypeProperty>
  <owl:DatatypeProperty rdf:about="http://example.org/onto/prop/yandex_mdb_kafka_cluster_file_delete_delay_ms">
    <rdfs:label>file_delete_delay_ms</rdfs:label>
    <rdfs:comment>The time to wait before deleting a file from the filesystem.</rdfs:comment>
    <rdfs:domain rdf:resource="http://example.org/onto/class/yandex_mdb_kafka_cluster"/>
    <rdfs:range rdf:resource="http://www.w3.org/2001/XMLSchema#string"/>
  </owl:DatatypeProperty>
  <owl:DatatypeProperty rdf:about="http://example.org/onto/prop/yandex_mdb_kafka_cluster_flush_messages">
    <rdfs:label>flush_messages</rdfs:label>
    <rdfs:comment>This setting allows specifying an interval at which we will force an fsync of data written to the log.</rdfs:comment>
    <rdfs:domain rdf:resource="http://example.org/onto/class/yandex_mdb_kafka_cluster"/>
    <rdfs:range rdf:resource="http://www.w3.org/2001/XMLSchema#string"/>
  </owl:DatatypeProperty>
  <owl:DatatypeProperty rdf:about="http://example.org/onto/prop/yandex_mdb_kafka_cluster_flush_ms">
    <rdfs:label>flush_ms</rdfs:label>
    <rdfs:comment>This setting allows specifying a time interval at which we will force an fsync of data written to the log.</rdfs:comment>
    <rdfs:domain rdf:resource="http://example.org/onto/class/yandex_mdb_kafka_cluster"/>
    <rdfs:range rdf:resource="http://www.w3.org/2001/XMLSchema#string"/>
  </owl:DatatypeProperty>
  <owl:DatatypeProperty rdf:about="http://example.org/onto/prop/yandex_mdb_kafka_cluster_max_message_bytes">
    <rdfs:label>max_message_bytes</rdfs:label>
    <rdfs:comment>The largest record batch size allowed by Kafka (after compression if compression is enabled).</rdfs:comment>
    <rdfs:domain rdf:resource="http://example.org/onto/class/yandex_mdb_kafka_cluster"/>
    <rdfs:range rdf:resource="http://www.w3.org/2001/XMLSchema#string"/>
  </owl:DatatypeProperty>
  <owl:DatatypeProperty rdf:about="http://example.org/onto/prop/yandex_mdb_kafka_cluster_min_compaction_lag_ms">
    <rdfs:label>min_compaction_lag_ms</rdfs:label>
    <rdfs:comment>The minimum time a message will remain uncompacted in the log. Only applicable for logs that are being compacted.</rdfs:comment>
    <rdfs:domain rdf:resource="http://example.org/onto/class/yandex_mdb_kafka_cluster"/>
    <rdfs:range rdf:resource="http://www.w3.org/2001/XMLSchema#string"/>
  </owl:DatatypeProperty>
  <owl:DatatypeProperty rdf:about="http://example.org/onto/prop/yandex_mdb_kafka_cluster_min_insync_replicas">
    <rdfs:label>min_insync_replicas</rdfs:label>
    <rdfs:comment>When a producer sets acks to "all" (or "-1"), this configuration specifies the minimum number of replicas that must acknowledge a write for the write to be considered successful.</rdfs:comment>
    <rdfs:domain rdf:resource="http://example.org/onto/class/yandex_mdb_kafka_cluster"/>
    <rdfs:range rdf:resource="http://www.w3.org/2001/XMLSchema#string"/>
  </owl:DatatypeProperty>
  <owl:DatatypeProperty rdf:about="http://example.org/onto/prop/yandex_mdb_kafka_cluster_preallocate">
    <rdfs:label>preallocate</rdfs:label>
    <rdfs:comment>True if we should preallocate the file on disk when creating a new log segment.</rdfs:comment>
    <rdfs:domain rdf:resource="http://example.org/onto/class/yandex_mdb_kafka_cluster"/>
    <rdfs:range rdf:resource="http://www.w3.org/2001/XMLSchema#string"/>
  </owl:DatatypeProperty>
  <owl:DatatypeProperty rdf:about="http://example.org/onto/prop/yandex_mdb_kafka_cluster_retention_bytes">
    <rdfs:label>retention_bytes</rdfs:label>
    <rdfs:comment>This configuration controls the maximum size a partition (which consists of log segments) can grow to before we will discard old log segments to free up space if we are using the "delete" retention policy.</rdfs:comment>
    <rdfs:domain rdf:resource="http://example.org/onto/class/yandex_mdb_kafka_cluster"/>
    <rdfs:range rdf:resource="http://www.w3.org/2001/XMLSchema#string"/>
  </owl:DatatypeProperty>
  <owl:DatatypeProperty rdf:about="http://example.org/onto/prop/yandex_mdb_kafka_cluster_retention_ms">
    <rdfs:label>retention_ms</rdfs:label>
    <rdfs:comment>This configuration controls the maximum time we will retain a log before we will discard old log segments to free up space if we are using the "delete" retention policy.</rdfs:comment>
    <rdfs:domain rdf:resource="http://example.org/onto/class/yandex_mdb_kafka_cluster"/>
    <rdfs:range rdf:resource="http://www.w3.org/2001/XMLSchema#string"/>
  </owl:DatatypeProperty>
  <owl:DatatypeProperty rdf:about="http://example.org/onto/prop/yandex_mdb_kafka_cluster_segment_bytes">
    <rdfs:label>segment_bytes</rdfs:label>
    <rdfs:comment>This configuration controls the segment file size for the log.</rdfs:comment>
    <rdfs:domain rdf:resource="http://example.org/onto/class/yandex_mdb_kafka_cluster"/>
    <rdfs:range rdf:resource="http://www.w3.org/2001/XMLSchema#string"/>
  </owl:DatatypeProperty>
  <owl:DatatypeProperty rdf:about="http://example.org/onto/prop/yandex_mdb_kafka_cluster_name">
    <rdfs:label>name</rdfs:label>
    <rdfs:comment>The name of the user.</rdfs:comment>
    <rdfs:domain rdf:resource="http://example.org/onto/class/yandex_mdb_kafka_cluster"/>
    <rdfs:range rdf:resource="http://www.w3.org/2001/XMLSchema#string"/>
  </owl:DatatypeProperty>
  <owl:DatatypeProperty rdf:about="http://example.org/onto/prop/yandex_mdb_kafka_cluster_password">
    <rdfs:label>password</rdfs:label>
    <rdfs:comment>The password of the user.</rdfs:comment>
    <rdfs:domain rdf:resource="http://example.org/onto/class/yandex_mdb_kafka_cluster"/>
    <rdfs:range rdf:resource="http://www.w3.org/2001/XMLSchema#string"/>
  </owl:DatatypeProperty>
  <owl:DatatypeProperty rdf:about="http://example.org/onto/prop/yandex_mdb_kafka_cluster_allow_hosts">
    <rdfs:label>allow_hosts</rdfs:label>
    <rdfs:comment>Set of hosts, to which this permission grants access to. Only ip-addresses allowed as value of single host.</rdfs:comment>
    <rdfs:domain rdf:resource="http://example.org/onto/class/yandex_mdb_kafka_cluster"/>
    <rdfs:range rdf:resource="http://www.w3.org/2001/XMLSchema#string"/>
  </owl:DatatypeProperty>
  <owl:DatatypeProperty rdf:about="http://example.org/onto/prop/yandex_mdb_kafka_cluster_role">
    <rdfs:label>role</rdfs:label>
    <rdfs:comment>The role type to grant to the topic.</rdfs:comment>
    <rdfs:domain rdf:resource="http://example.org/onto/class/yandex_mdb_kafka_cluster"/>
    <rdfs:range rdf:resource="http://www.w3.org/2001/XMLSchema#string"/>
  </owl:DatatypeProperty>
  <owl:DatatypeProperty rdf:about="http://example.org/onto/prop/yandex_mdb_kafka_cluster_topic_name">
    <rdfs:label>topic_name</rdfs:label>
    <rdfs:comment>The name of the topic that the permission grants access to.</rdfs:comment>
    <rdfs:domain rdf:resource="http://example.org/onto/class/yandex_mdb_kafka_cluster"/>
    <rdfs:range rdf:resource="http://www.w3.org/2001/XMLSchema#string"/>
  </owl:DatatypeProperty>
</rdf:RDF>
