<?xml version="1.0" encoding="UTF-8"?>
<rdf:RDF
  xmlns:rdf="http://www.w3.org/1999/02/22-rdf-syntax-ns#"
  xmlns:rdfs="http://www.w3.org/2000/01/rdf-schema#"
  xmlns:owl="http://www.w3.org/2002/07/owl#"
  xmlns:xsd="http://www.w3.org/2001/XMLSchema#"
  xml:base="http://example.org/onto/">
  <owl:Class rdf:about="http://example.org/onto/class/yandex_iam_workload_identity_oidc_federation">
    <rdfs:label>yandex_iam_workload_identity_oidc_federation</rdfs:label>
    <rdfs:comment>A OIDC workload identity federation.</rdfs:comment>
  </owl:Class>
  <owl:DatatypeProperty rdf:about="http://example.org/onto/prop/yandex_iam_workload_identity_oidc_federation_audiences">
    <rdfs:label>audiences</rdfs:label>
    <rdfs:comment>List of trusted values for aud claim.</rdfs:comment>
    <rdfs:domain rdf:resource="http://example.org/onto/class/yandex_iam_workload_identity_oidc_federation"/>
    <rdfs:range rdf:resource="http://www.w3.org/2001/XMLSchema#string"/>
  </owl:DatatypeProperty>
  <owl:DatatypeProperty rdf:about="http://example.org/onto/prop/yandex_iam_workload_identity_oidc_federation_created_at">
    <rdfs:label>created_at</rdfs:label>
    <rdfs:comment>Creation timestamp.</rdfs:comment>
    <rdfs:domain rdf:resource="http://example.org/onto/class/yandex_iam_workload_identity_oidc_federation"/>
    <rdfs:range rdf:resource="http://www.w3.org/2001/XMLSchema#string"/>
  </owl:DatatypeProperty>
  <owl:DatatypeProperty rdf:about="http://example.org/onto/prop/yandex_iam_workload_identity_oidc_federation_description">
    <rdfs:label>description</rdfs:label>
    <rdfs:comment>Description of the service account. 0-256 characters long.</rdfs:comment>
    <rdfs:domain rdf:resource="http://example.org/onto/class/yandex_iam_workload_identity_oidc_federation"/>
    <rdfs:range rdf:resource="http://www.w3.org/2001/XMLSchema#string"/>
  </owl:DatatypeProperty>
  <owl:DatatypeProperty rdf:about="http://example.org/onto/prop/yandex_iam_workload_identity_oidc_federation_disabled">
    <rdfs:label>disabled</rdfs:label>
    <rdfs:comment>True - the OIDC workload identity federation is disabled and cannot be used for authentication.
 False - the OIDC workload identity federation is enabled and can be used for authentication.</rdfs:comment>
    <rdfs:domain rdf:resource="http://example.org/onto/class/yandex_iam_workload_identity_oidc_federation"/>
    <rdfs:range rdf:resource="http://www.w3.org/2001/XMLSchema#string"/>
  </owl:DatatypeProperty>
  <owl:DatatypeProperty rdf:about="http://example.org/onto/prop/yandex_iam_workload_identity_oidc_federation_enabled">
    <rdfs:label>enabled</rdfs:label>
    <rdfs:comment>True - the OIDC workload identity federation is enabled and can be used for authentication.
 False - the OIDC workload identity federation is disabled and cannot be used for authentication.</rdfs:comment>
    <rdfs:domain rdf:resource="http://example.org/onto/class/yandex_iam_workload_identity_oidc_federation"/>
    <rdfs:range rdf:resource="http://www.w3.org/2001/XMLSchema#string"/>
  </owl:DatatypeProperty>
  <owl:DatatypeProperty rdf:about="http://example.org/onto/prop/yandex_iam_workload_identity_oidc_federation_federation_id">
    <rdfs:label>federation_id</rdfs:label>
    <rdfs:comment>ID of the OIDC workload identity federation to return.
 To get the OIDC workload identity federation ID, make a [FederationService.List] request.</rdfs:comment>
    <rdfs:domain rdf:resource="http://example.org/onto/class/yandex_iam_workload_identity_oidc_federation"/>
    <rdfs:range rdf:resource="http://www.w3.org/2001/XMLSchema#string"/>
  </owl:DatatypeProperty>
  <owl:DatatypeProperty rdf:about="http://example.org/onto/prop/yandex_iam_workload_identity_oidc_federation_folder_id">
    <rdfs:label>folder_id</rdfs:label>
    <rdfs:comment>ID of the folder that the OIDC workload identity federation belongs to.</rdfs:comment>
    <rdfs:domain rdf:resource="http://example.org/onto/class/yandex_iam_workload_identity_oidc_federation"/>
    <rdfs:range rdf:resource="http://www.w3.org/2001/XMLSchema#string"/>
  </owl:DatatypeProperty>
  <owl:DatatypeProperty rdf:about="http://example.org/onto/prop/yandex_iam_workload_identity_oidc_federation_id">
    <rdfs:label>id</rdfs:label>
    <rdfs:comment>ID of the OIDC workload identity federation to return.
 To get the OIDC workload identity federation ID, make a [FederationService.List] request.</rdfs:comment>
    <rdfs:domain rdf:resource="http://example.org/onto/class/yandex_iam_workload_identity_oidc_federation"/>
    <rdfs:range rdf:resource="http://www.w3.org/2001/XMLSchema#string"/>
  </owl:DatatypeProperty>
  <owl:DatatypeProperty rdf:about="http://example.org/onto/prop/yandex_iam_workload_identity_oidc_federation_issuer">
    <rdfs:label>issuer</rdfs:label>
    <rdfs:comment>URL of the external IdP server to be used for authentication.</rdfs:comment>
    <rdfs:domain rdf:resource="http://example.org/onto/class/yandex_iam_workload_identity_oidc_federation"/>
    <rdfs:range rdf:resource="http://www.w3.org/2001/XMLSchema#string"/>
  </owl:DatatypeProperty>
  <owl:DatatypeProperty rdf:about="http://example.org/onto/prop/yandex_iam_workload_identity_oidc_federation_jwks_url">
    <rdfs:label>jwks_url</rdfs:label>
    <rdfs:comment>URL reference to trusted keys in format of JSON Web Key Set.</rdfs:comment>
    <rdfs:domain rdf:resource="http://example.org/onto/class/yandex_iam_workload_identity_oidc_federation"/>
    <rdfs:range rdf:resource="http://www.w3.org/2001/XMLSchema#string"/>
  </owl:DatatypeProperty>
  <owl:DatatypeProperty rdf:about="http://example.org/onto/prop/yandex_iam_workload_identity_oidc_federation_labels">
    <rdfs:label>labels</rdfs:label>
    <rdfs:comment>Resource labels as `` key:value `` pairs</rdfs:comment>
    <rdfs:domain rdf:resource="http://example.org/onto/class/yandex_iam_workload_identity_oidc_federation"/>
    <rdfs:range rdf:resource="http://www.w3.org/2001/XMLSchema#string"/>
  </owl:DatatypeProperty>
  <owl:DatatypeProperty rdf:about="http://example.org/onto/prop/yandex_iam_workload_identity_oidc_federation_name">
    <rdfs:label>name</rdfs:label>
    <rdfs:comment>Name of the OIDC workload identity federation
 The name is unique within the folder. 3-63 characters long.</rdfs:comment>
    <rdfs:domain rdf:resource="http://example.org/onto/class/yandex_iam_workload_identity_oidc_federation"/>
    <rdfs:range rdf:resource="http://www.w3.org/2001/XMLSchema#string"/>
  </owl:DatatypeProperty>
  <owl:DatatypeProperty rdf:about="http://example.org/onto/prop/yandex_iam_workload_identity_oidc_federation_create">
    <rdfs:label>create</rdfs:label>
    <rdfs:comment>A string that can be [parsed as a duration](https://pkg.go.dev/time#ParseDuration) consisting of numbers and unit suffixes, such as "30s" or "2h45m". Valid time units are "s" (seconds), "m" (minutes), "h" (hours).</rdfs:comment>
    <rdfs:domain rdf:resource="http://example.org/onto/class/yandex_iam_workload_identity_oidc_federation"/>
    <rdfs:range rdf:resource="http://www.w3.org/2001/XMLSchema#string"/>
  </owl:DatatypeProperty>
  <owl:DatatypeProperty rdf:about="http://example.org/onto/prop/yandex_iam_workload_identity_oidc_federation_delete">
    <rdfs:label>delete</rdfs:label>
    <rdfs:comment>A string that can be [parsed as a duration](https://pkg.go.dev/time#ParseDuration) consisting of numbers and unit suffixes, such as "30s" or "2h45m". Valid time units are "s" (seconds), "m" (minutes), "h" (hours). Setting a timeout for a Delete operation is only applicable if changes are saved into state before the destroy operation occurs.</rdfs:comment>
    <rdfs:domain rdf:resource="http://example.org/onto/class/yandex_iam_workload_identity_oidc_federation"/>
    <rdfs:range rdf:resource="http://www.w3.org/2001/XMLSchema#string"/>
  </owl:DatatypeProperty>
  <owl:DatatypeProperty rdf:about="http://example.org/onto/prop/yandex_iam_workload_identity_oidc_federation_read">
    <rdfs:label>read</rdfs:label>
    <rdfs:comment>A string that can be [parsed as a duration](https://pkg.go.dev/time#ParseDuration) consisting of numbers and unit suffixes, such as "30s" or "2h45m". Valid time units are "s" (seconds), "m" (minutes), "h" (hours). Read operations occur during any refresh or planning operation when refresh is enabled.</rdfs:comment>
    <rdfs:domain rdf:resource="http://example.org/onto/class/yandex_iam_workload_identity_oidc_federation"/>
    <rdfs:range rdf:resource="http://www.w3.org/2001/XMLSchema#string"/>
  </owl:DatatypeProperty>
  <owl:DatatypeProperty rdf:about="http://example.org/onto/prop/yandex_iam_workload_identity_oidc_federation_update">
    <rdfs:label>update</rdfs:label>
    <rdfs:comment>A string that can be [parsed as a duration](https://pkg.go.dev/time#ParseDuration) consisting of numbers and unit suffixes, such as "30s" or "2h45m". Valid time units are "s" (seconds), "m" (minutes), "h" (hours).</rdfs:comment>
    <rdfs:domain rdf:resource="http://example.org/onto/class/yandex_iam_workload_identity_oidc_federation"/>
    <rdfs:range rdf:resource="http://www.w3.org/2001/XMLSchema#string"/>
  </owl:DatatypeProperty>
</rdf:RDF>
