<?xml version="1.0" encoding="UTF-8"?>
<rdf:RDF
  xmlns:rdf="http://www.w3.org/1999/02/22-rdf-syntax-ns#"
  xmlns:rdfs="http://www.w3.org/2000/01/rdf-schema#"
  xmlns:owl="http://www.w3.org/2002/07/owl#"
  xmlns:xsd="http://www.w3.org/2001/XMLSchema#"
  xml:base="http://example.org/onto/">
  <owl:Class rdf:about="http://example.org/onto/class/yandex_ydb_database_dedicated">
    <rdfs:label>yandex_ydb_database_dedicated</rdfs:label>
    <rdfs:comment>Yandex Database (dedicated) resource. For more information, see [the official documentation](https://yandex.cloud/docs/ydb/concepts/serverless_and_dedicated).</rdfs:comment>
  </owl:Class>
  <owl:DatatypeProperty rdf:about="http://example.org/onto/prop/yandex_ydb_database_dedicated_assign_public_ips">
    <rdfs:label>assign_public_ips</rdfs:label>
    <rdfs:comment>Whether public IP addresses should be assigned to the Yandex Database cluster.</rdfs:comment>
    <rdfs:domain rdf:resource="http://example.org/onto/class/yandex_ydb_database_dedicated"/>
    <rdfs:range rdf:resource="http://www.w3.org/2001/XMLSchema#string"/>
  </owl:DatatypeProperty>
  <owl:DatatypeProperty rdf:about="http://example.org/onto/prop/yandex_ydb_database_dedicated_created_at">
    <rdfs:label>created_at</rdfs:label>
    <rdfs:comment>The creation timestamp of the resource.</rdfs:comment>
    <rdfs:domain rdf:resource="http://example.org/onto/class/yandex_ydb_database_dedicated"/>
    <rdfs:range rdf:resource="http://www.w3.org/2001/XMLSchema#string"/>
  </owl:DatatypeProperty>
  <owl:DatatypeProperty rdf:about="http://example.org/onto/prop/yandex_ydb_database_dedicated_database_path">
    <rdfs:label>database_path</rdfs:label>
    <rdfs:comment>Full database path of the Yandex Database cluster. Useful for SDK configuration.</rdfs:comment>
    <rdfs:domain rdf:resource="http://example.org/onto/class/yandex_ydb_database_dedicated"/>
    <rdfs:range rdf:resource="http://www.w3.org/2001/XMLSchema#string"/>
  </owl:DatatypeProperty>
  <owl:DatatypeProperty rdf:about="http://example.org/onto/prop/yandex_ydb_database_dedicated_deletion_protection">
    <rdfs:label>deletion_protection</rdfs:label>
    <rdfs:comment>The `true` value means that resource is protected from accidental deletion.</rdfs:comment>
    <rdfs:domain rdf:resource="http://example.org/onto/class/yandex_ydb_database_dedicated"/>
    <rdfs:range rdf:resource="http://www.w3.org/2001/XMLSchema#string"/>
  </owl:DatatypeProperty>
  <owl:DatatypeProperty rdf:about="http://example.org/onto/prop/yandex_ydb_database_dedicated_description">
    <rdfs:label>description</rdfs:label>
    <rdfs:comment>The resource description.</rdfs:comment>
    <rdfs:domain rdf:resource="http://example.org/onto/class/yandex_ydb_database_dedicated"/>
    <rdfs:range rdf:resource="http://www.w3.org/2001/XMLSchema#string"/>
  </owl:DatatypeProperty>
  <owl:DatatypeProperty rdf:about="http://example.org/onto/prop/yandex_ydb_database_dedicated_folder_id">
    <rdfs:label>folder_id</rdfs:label>
    <rdfs:comment>The folder identifier that resource belongs to. If it is not provided, the default provider `folder-id` is used.</rdfs:comment>
    <rdfs:domain rdf:resource="http://example.org/onto/class/yandex_ydb_database_dedicated"/>
    <rdfs:range rdf:resource="http://www.w3.org/2001/XMLSchema#string"/>
  </owl:DatatypeProperty>
  <owl:DatatypeProperty rdf:about="http://example.org/onto/prop/yandex_ydb_database_dedicated_id">
    <rdfs:label>id</rdfs:label>
    <rdfs:domain rdf:resource="http://example.org/onto/class/yandex_ydb_database_dedicated"/>
    <rdfs:range rdf:resource="http://www.w3.org/2001/XMLSchema#string"/>
  </owl:DatatypeProperty>
  <owl:DatatypeProperty rdf:about="http://example.org/onto/prop/yandex_ydb_database_dedicated_labels">
    <rdfs:label>labels</rdfs:label>
    <rdfs:comment>A set of key/value label pairs which assigned to resource.</rdfs:comment>
    <rdfs:domain rdf:resource="http://example.org/onto/class/yandex_ydb_database_dedicated"/>
    <rdfs:range rdf:resource="http://www.w3.org/2001/XMLSchema#string"/>
  </owl:DatatypeProperty>
  <owl:DatatypeProperty rdf:about="http://example.org/onto/prop/yandex_ydb_database_dedicated_location_id">
    <rdfs:label>location_id</rdfs:label>
    <rdfs:comment>Location ID for the Yandex Database cluster.</rdfs:comment>
    <rdfs:domain rdf:resource="http://example.org/onto/class/yandex_ydb_database_dedicated"/>
    <rdfs:range rdf:resource="http://www.w3.org/2001/XMLSchema#string"/>
  </owl:DatatypeProperty>
  <owl:DatatypeProperty rdf:about="http://example.org/onto/prop/yandex_ydb_database_dedicated_name">
    <rdfs:label>name</rdfs:label>
    <rdfs:comment>The resource name.</rdfs:comment>
    <rdfs:domain rdf:resource="http://example.org/onto/class/yandex_ydb_database_dedicated"/>
    <rdfs:range rdf:resource="http://www.w3.org/2001/XMLSchema#string"/>
  </owl:DatatypeProperty>
  <owl:DatatypeProperty rdf:about="http://example.org/onto/prop/yandex_ydb_database_dedicated_network_id">
    <rdfs:label>network_id</rdfs:label>
    <rdfs:comment>The `VPC Network ID` of subnets which resource attached to.</rdfs:comment>
    <rdfs:domain rdf:resource="http://example.org/onto/class/yandex_ydb_database_dedicated"/>
    <rdfs:range rdf:resource="http://www.w3.org/2001/XMLSchema#string"/>
  </owl:DatatypeProperty>
  <owl:DatatypeProperty rdf:about="http://example.org/onto/prop/yandex_ydb_database_dedicated_resource_preset_id">
    <rdfs:label>resource_preset_id</rdfs:label>
    <rdfs:comment>The Yandex Database cluster preset. Available presets can be obtained via `yc ydb resource-preset list` command.</rdfs:comment>
    <rdfs:domain rdf:resource="http://example.org/onto/class/yandex_ydb_database_dedicated"/>
    <rdfs:range rdf:resource="http://www.w3.org/2001/XMLSchema#string"/>
  </owl:DatatypeProperty>
  <owl:DatatypeProperty rdf:about="http://example.org/onto/prop/yandex_ydb_database_dedicated_security_group_ids">
    <rdfs:label>security_group_ids</rdfs:label>
    <rdfs:comment>The list of security groups applied to resource or their components.</rdfs:comment>
    <rdfs:domain rdf:resource="http://example.org/onto/class/yandex_ydb_database_dedicated"/>
    <rdfs:range rdf:resource="http://www.w3.org/2001/XMLSchema#string"/>
  </owl:DatatypeProperty>
  <owl:DatatypeProperty rdf:about="http://example.org/onto/prop/yandex_ydb_database_dedicated_sleep_after">
    <rdfs:label>sleep_after</rdfs:label>
    <rdfs:domain rdf:resource="http://example.org/onto/class/yandex_ydb_database_dedicated"/>
    <rdfs:range rdf:resource="http://www.w3.org/2001/XMLSchema#string"/>
  </owl:DatatypeProperty>
  <owl:DatatypeProperty rdf:about="http://example.org/onto/prop/yandex_ydb_database_dedicated_status">
    <rdfs:label>status</rdfs:label>
    <rdfs:comment>Status of the Yandex Database cluster.</rdfs:comment>
    <rdfs:domain rdf:resource="http://example.org/onto/class/yandex_ydb_database_dedicated"/>
    <rdfs:range rdf:resource="http://www.w3.org/2001/XMLSchema#string"/>
  </owl:DatatypeProperty>
  <owl:DatatypeProperty rdf:about="http://example.org/onto/prop/yandex_ydb_database_dedicated_subnet_ids">
    <rdfs:label>subnet_ids</rdfs:label>
    <rdfs:comment>The list of VPC subnets identifiers which resource is attached.</rdfs:comment>
    <rdfs:domain rdf:resource="http://example.org/onto/class/yandex_ydb_database_dedicated"/>
    <rdfs:range rdf:resource="http://www.w3.org/2001/XMLSchema#string"/>
  </owl:DatatypeProperty>
  <owl:DatatypeProperty rdf:about="http://example.org/onto/prop/yandex_ydb_database_dedicated_tls_enabled">
    <rdfs:label>tls_enabled</rdfs:label>
    <rdfs:comment>Whether TLS is enabled for the Yandex Database cluster. Useful for SDK configuration.</rdfs:comment>
    <rdfs:domain rdf:resource="http://example.org/onto/class/yandex_ydb_database_dedicated"/>
    <rdfs:range rdf:resource="http://www.w3.org/2001/XMLSchema#string"/>
  </owl:DatatypeProperty>
  <owl:DatatypeProperty rdf:about="http://example.org/onto/prop/yandex_ydb_database_dedicated_ydb_api_endpoint">
    <rdfs:label>ydb_api_endpoint</rdfs:label>
    <rdfs:comment>API endpoint of the Yandex Database cluster. Useful for SDK configuration.</rdfs:comment>
    <rdfs:domain rdf:resource="http://example.org/onto/class/yandex_ydb_database_dedicated"/>
    <rdfs:range rdf:resource="http://www.w3.org/2001/XMLSchema#string"/>
  </owl:DatatypeProperty>
  <owl:DatatypeProperty rdf:about="http://example.org/onto/prop/yandex_ydb_database_dedicated_ydb_full_endpoint">
    <rdfs:label>ydb_full_endpoint</rdfs:label>
    <rdfs:comment>Full endpoint of the Yandex Database cluster.</rdfs:comment>
    <rdfs:domain rdf:resource="http://example.org/onto/class/yandex_ydb_database_dedicated"/>
    <rdfs:range rdf:resource="http://www.w3.org/2001/XMLSchema#string"/>
  </owl:DatatypeProperty>
  <owl:DatatypeProperty rdf:about="http://example.org/onto/prop/yandex_ydb_database_dedicated_id">
    <rdfs:label>id</rdfs:label>
    <rdfs:comment>Region ID for the Yandex Database cluster.</rdfs:comment>
    <rdfs:domain rdf:resource="http://example.org/onto/class/yandex_ydb_database_dedicated"/>
    <rdfs:range rdf:resource="http://www.w3.org/2001/XMLSchema#string"/>
  </owl:DatatypeProperty>
  <owl:DatatypeProperty rdf:about="http://example.org/onto/prop/yandex_ydb_database_dedicated_max_size">
    <rdfs:label>max_size</rdfs:label>
    <rdfs:comment>Maximum number of nodes to which autoscaling can scale the database.</rdfs:comment>
    <rdfs:domain rdf:resource="http://example.org/onto/class/yandex_ydb_database_dedicated"/>
    <rdfs:range rdf:resource="http://www.w3.org/2001/XMLSchema#string"/>
  </owl:DatatypeProperty>
  <owl:DatatypeProperty rdf:about="http://example.org/onto/prop/yandex_ydb_database_dedicated_min_size">
    <rdfs:label>min_size</rdfs:label>
    <rdfs:comment>Minimum number of nodes to which autoscaling can scale the database.</rdfs:comment>
    <rdfs:domain rdf:resource="http://example.org/onto/class/yandex_ydb_database_dedicated"/>
    <rdfs:range rdf:resource="http://www.w3.org/2001/XMLSchema#string"/>
  </owl:DatatypeProperty>
  <owl:DatatypeProperty rdf:about="http://example.org/onto/prop/yandex_ydb_database_dedicated_cpu_utilization_percent">
    <rdfs:label>cpu_utilization_percent</rdfs:label>
    <rdfs:comment>A percentage of database nodes average CPU utilization.</rdfs:comment>
    <rdfs:domain rdf:resource="http://example.org/onto/class/yandex_ydb_database_dedicated"/>
    <rdfs:range rdf:resource="http://www.w3.org/2001/XMLSchema#string"/>
  </owl:DatatypeProperty>
  <owl:DatatypeProperty rdf:about="http://example.org/onto/prop/yandex_ydb_database_dedicated_size">
    <rdfs:label>size</rdfs:label>
    <rdfs:comment>Number of instances for the Yandex Database cluster.</rdfs:comment>
    <rdfs:domain rdf:resource="http://example.org/onto/class/yandex_ydb_database_dedicated"/>
    <rdfs:range rdf:resource="http://www.w3.org/2001/XMLSchema#string"/>
  </owl:DatatypeProperty>
  <owl:DatatypeProperty rdf:about="http://example.org/onto/prop/yandex_ydb_database_dedicated_group_count">
    <rdfs:label>group_count</rdfs:label>
    <rdfs:comment>Amount of storage groups of selected type for the Yandex Database cluster.</rdfs:comment>
    <rdfs:domain rdf:resource="http://example.org/onto/class/yandex_ydb_database_dedicated"/>
    <rdfs:range rdf:resource="http://www.w3.org/2001/XMLSchema#string"/>
  </owl:DatatypeProperty>
  <owl:DatatypeProperty rdf:about="http://example.org/onto/prop/yandex_ydb_database_dedicated_storage_type_id">
    <rdfs:label>storage_type_id</rdfs:label>
    <rdfs:comment>Storage type ID for the Yandex Database cluster. Available presets can be obtained via `yc ydb storage-type list` command.</rdfs:comment>
    <rdfs:domain rdf:resource="http://example.org/onto/class/yandex_ydb_database_dedicated"/>
    <rdfs:range rdf:resource="http://www.w3.org/2001/XMLSchema#string"/>
  </owl:DatatypeProperty>
  <owl:DatatypeProperty rdf:about="http://example.org/onto/prop/yandex_ydb_database_dedicated_default">
    <rdfs:label>default</rdfs:label>
    <rdfs:domain rdf:resource="http://example.org/onto/class/yandex_ydb_database_dedicated"/>
    <rdfs:range rdf:resource="http://www.w3.org/2001/XMLSchema#string"/>
  </owl:DatatypeProperty>
</rdf:RDF>
