<?xml version="1.0" encoding="UTF-8"?>
<rdf:RDF
  xmlns:rdf="http://www.w3.org/1999/02/22-rdf-syntax-ns#"
  xmlns:rdfs="http://www.w3.org/2000/01/rdf-schema#"
  xmlns:owl="http://www.w3.org/2002/07/owl#"
  xmlns:xsd="http://www.w3.org/2001/XMLSchema#"
  xml:base="http://example.org/onto/">
  <owl:Class rdf:about="http://example.org/onto/class/yandex_vpc_security_group_rule">
    <rdfs:label>yandex_vpc_security_group_rule</rdfs:label>
    <rdfs:comment>Manages `Security Group Rule` within the Yandex Cloud. For more information, see [Documentation](https://yandex.cloud/docs/vpc/concepts/security-groups).

~> There is another way to manage security group rules by `ingress` and `egress` arguments in `yandex_vpc_security_group` resource. Both ways are similar but not compatible with each other. Using `Security Group Rule` at the same time with `yandex_vpc_security_group` resource will cause a conflict of rules configuration and it's not recommended!

~> Either one `port` argument or both `from_port` and `to_port` arguments can be specified.

~> If `port` or `from_port`/`to_port` aren't specified or set by -1, ANY port will be sent.
~> Can't use specified port if protocol is one of `ICMP` or `IPV6_ICMP`.

~> One of arguments `v4_cidr_blocks`/`v6_cidr_blocks` or `predefined_target` or `security_group_id` must be specified.</rdfs:comment>
  </owl:Class>
  <owl:DatatypeProperty rdf:about="http://example.org/onto/prop/yandex_vpc_security_group_rule_description">
    <rdfs:label>description</rdfs:label>
    <rdfs:comment>The resource description.</rdfs:comment>
    <rdfs:domain rdf:resource="http://example.org/onto/class/yandex_vpc_security_group_rule"/>
    <rdfs:range rdf:resource="http://www.w3.org/2001/XMLSchema#string"/>
  </owl:DatatypeProperty>
  <owl:DatatypeProperty rdf:about="http://example.org/onto/prop/yandex_vpc_security_group_rule_direction">
    <rdfs:label>direction</rdfs:label>
    <rdfs:comment>Direction of the Security group rule. Can be `ingress` (inbound network traffic to the VPC network) or `egress` (outbound network traffic from the VPC network).</rdfs:comment>
    <rdfs:domain rdf:resource="http://example.org/onto/class/yandex_vpc_security_group_rule"/>
    <rdfs:range rdf:resource="http://www.w3.org/2001/XMLSchema#string"/>
  </owl:DatatypeProperty>
  <owl:DatatypeProperty rdf:about="http://example.org/onto/prop/yandex_vpc_security_group_rule_from_port">
    <rdfs:label>from_port</rdfs:label>
    <rdfs:comment>Minimum port number. Applicable for TCP and UDP protocols.</rdfs:comment>
    <rdfs:domain rdf:resource="http://example.org/onto/class/yandex_vpc_security_group_rule"/>
    <rdfs:range rdf:resource="http://www.w3.org/2001/XMLSchema#string"/>
  </owl:DatatypeProperty>
  <owl:DatatypeProperty rdf:about="http://example.org/onto/prop/yandex_vpc_security_group_rule_id">
    <rdfs:label>id</rdfs:label>
    <rdfs:comment>The resource identifier.</rdfs:comment>
    <rdfs:domain rdf:resource="http://example.org/onto/class/yandex_vpc_security_group_rule"/>
    <rdfs:range rdf:resource="http://www.w3.org/2001/XMLSchema#string"/>
  </owl:DatatypeProperty>
  <owl:DatatypeProperty rdf:about="http://example.org/onto/prop/yandex_vpc_security_group_rule_labels">
    <rdfs:label>labels</rdfs:label>
    <rdfs:comment>A set of key/value label pairs which assigned to resource.</rdfs:comment>
    <rdfs:domain rdf:resource="http://example.org/onto/class/yandex_vpc_security_group_rule"/>
    <rdfs:range rdf:resource="http://www.w3.org/2001/XMLSchema#string"/>
  </owl:DatatypeProperty>
  <owl:DatatypeProperty rdf:about="http://example.org/onto/prop/yandex_vpc_security_group_rule_port">
    <rdfs:label>port</rdfs:label>
    <rdfs:comment>Port number (if applied to a single port).</rdfs:comment>
    <rdfs:domain rdf:resource="http://example.org/onto/class/yandex_vpc_security_group_rule"/>
    <rdfs:range rdf:resource="http://www.w3.org/2001/XMLSchema#string"/>
  </owl:DatatypeProperty>
  <owl:DatatypeProperty rdf:about="http://example.org/onto/prop/yandex_vpc_security_group_rule_predefined_target">
    <rdfs:label>predefined_target</rdfs:label>
    <rdfs:comment>Special-purpose targets. The `self_security_group` target refers to this particular security group. The `loadbalancer_healthchecks` target represents [NLB health check nodes](https://yandex.cloud/docs/network-load-balancer/concepts/health-check).</rdfs:comment>
    <rdfs:domain rdf:resource="http://example.org/onto/class/yandex_vpc_security_group_rule"/>
    <rdfs:range rdf:resource="http://www.w3.org/2001/XMLSchema#string"/>
  </owl:DatatypeProperty>
  <owl:DatatypeProperty rdf:about="http://example.org/onto/prop/yandex_vpc_security_group_rule_protocol">
    <rdfs:label>protocol</rdfs:label>
    <rdfs:comment>Specific network protocol. Can be one of `ANY`, `TCP`, `UDP`, `ICMP`, `IPV6_ICMP`.</rdfs:comment>
    <rdfs:domain rdf:resource="http://example.org/onto/class/yandex_vpc_security_group_rule"/>
    <rdfs:range rdf:resource="http://www.w3.org/2001/XMLSchema#string"/>
  </owl:DatatypeProperty>
  <owl:DatatypeProperty rdf:about="http://example.org/onto/prop/yandex_vpc_security_group_rule_security_group_binding">
    <rdfs:label>security_group_binding</rdfs:label>
    <rdfs:comment>The id of target security group which rule belongs to.</rdfs:comment>
    <rdfs:domain rdf:resource="http://example.org/onto/class/yandex_vpc_security_group_rule"/>
    <rdfs:range rdf:resource="http://www.w3.org/2001/XMLSchema#string"/>
  </owl:DatatypeProperty>
  <owl:DatatypeProperty rdf:about="http://example.org/onto/prop/yandex_vpc_security_group_rule_security_group_id">
    <rdfs:label>security_group_id</rdfs:label>
    <rdfs:comment>Target security group ID for this Security group rule.</rdfs:comment>
    <rdfs:domain rdf:resource="http://example.org/onto/class/yandex_vpc_security_group_rule"/>
    <rdfs:range rdf:resource="http://www.w3.org/2001/XMLSchema#string"/>
  </owl:DatatypeProperty>
  <owl:DatatypeProperty rdf:about="http://example.org/onto/prop/yandex_vpc_security_group_rule_to_port">
    <rdfs:label>to_port</rdfs:label>
    <rdfs:comment>Maximum port number. Applicable for TCP and UDP protocols.</rdfs:comment>
    <rdfs:domain rdf:resource="http://example.org/onto/class/yandex_vpc_security_group_rule"/>
    <rdfs:range rdf:resource="http://www.w3.org/2001/XMLSchema#string"/>
  </owl:DatatypeProperty>
  <owl:DatatypeProperty rdf:about="http://example.org/onto/prop/yandex_vpc_security_group_rule_v4_cidr_blocks">
    <rdfs:label>v4_cidr_blocks</rdfs:label>
    <rdfs:comment>The list of IPv4 CIDR prefixes for this Security group rule.</rdfs:comment>
    <rdfs:domain rdf:resource="http://example.org/onto/class/yandex_vpc_security_group_rule"/>
    <rdfs:range rdf:resource="http://www.w3.org/2001/XMLSchema#string"/>
  </owl:DatatypeProperty>
  <owl:DatatypeProperty rdf:about="http://example.org/onto/prop/yandex_vpc_security_group_rule_v6_cidr_blocks">
    <rdfs:label>v6_cidr_blocks</rdfs:label>
    <rdfs:comment>The list of IPv6 CIDR prefixes for this Security group rule. Not supported yet.</rdfs:comment>
    <rdfs:domain rdf:resource="http://example.org/onto/class/yandex_vpc_security_group_rule"/>
    <rdfs:range rdf:resource="http://www.w3.org/2001/XMLSchema#string"/>
  </owl:DatatypeProperty>
  <owl:DatatypeProperty rdf:about="http://example.org/onto/prop/yandex_vpc_security_group_rule_create">
    <rdfs:label>create</rdfs:label>
    <rdfs:comment>A string that can be [parsed as a duration](https://pkg.go.dev/time#ParseDuration) consisting of numbers and unit suffixes, such as "30s" or "2h45m". Valid time units are "s" (seconds), "m" (minutes), "h" (hours).</rdfs:comment>
    <rdfs:domain rdf:resource="http://example.org/onto/class/yandex_vpc_security_group_rule"/>
    <rdfs:range rdf:resource="http://www.w3.org/2001/XMLSchema#string"/>
  </owl:DatatypeProperty>
  <owl:DatatypeProperty rdf:about="http://example.org/onto/prop/yandex_vpc_security_group_rule_delete">
    <rdfs:label>delete</rdfs:label>
    <rdfs:comment>A string that can be [parsed as a duration](https://pkg.go.dev/time#ParseDuration) consisting of numbers and unit suffixes, such as "30s" or "2h45m". Valid time units are "s" (seconds), "m" (minutes), "h" (hours). Setting a timeout for a Delete operation is only applicable if changes are saved into state before the destroy operation occurs.</rdfs:comment>
    <rdfs:domain rdf:resource="http://example.org/onto/class/yandex_vpc_security_group_rule"/>
    <rdfs:range rdf:resource="http://www.w3.org/2001/XMLSchema#string"/>
  </owl:DatatypeProperty>
  <owl:DatatypeProperty rdf:about="http://example.org/onto/prop/yandex_vpc_security_group_rule_update">
    <rdfs:label>update</rdfs:label>
    <rdfs:comment>A string that can be [parsed as a duration](https://pkg.go.dev/time#ParseDuration) consisting of numbers and unit suffixes, such as "30s" or "2h45m". Valid time units are "s" (seconds), "m" (minutes), "h" (hours).</rdfs:comment>
    <rdfs:domain rdf:resource="http://example.org/onto/class/yandex_vpc_security_group_rule"/>
    <rdfs:range rdf:resource="http://www.w3.org/2001/XMLSchema#string"/>
  </owl:DatatypeProperty>
</rdf:RDF>
