<?xml version="1.0" encoding="UTF-8"?>
<rdf:RDF
  xmlns:rdf="http://www.w3.org/1999/02/22-rdf-syntax-ns#"
  xmlns:rdfs="http://www.w3.org/2000/01/rdf-schema#"
  xmlns:owl="http://www.w3.org/2002/07/owl#"
  xmlns:xsd="http://www.w3.org/2001/XMLSchema#"
  xml:base="http://example.org/onto/">
  <owl:Class rdf:about="http://example.org/onto/class/yandex_mdb_clickhouse_cluster">
    <rdfs:label>yandex_mdb_clickhouse_cluster</rdfs:label>
    <rdfs:comment>Manages a ClickHouse cluster within the Yandex Cloud. For more information, see [the official documentation](https://yandex.cloud/docs/managed-clickhouse/concepts).</rdfs:comment>
  </owl:Class>
  <owl:DatatypeProperty rdf:about="http://example.org/onto/prop/yandex_mdb_clickhouse_cluster_admin_password">
    <rdfs:label>admin_password</rdfs:label>
    <rdfs:comment>A password used to authorize as user `admin` when `sql_user_management` enabled.</rdfs:comment>
    <rdfs:domain rdf:resource="http://example.org/onto/class/yandex_mdb_clickhouse_cluster"/>
    <rdfs:range rdf:resource="http://www.w3.org/2001/XMLSchema#string"/>
  </owl:DatatypeProperty>
  <owl:DatatypeProperty rdf:about="http://example.org/onto/prop/yandex_mdb_clickhouse_cluster_backup_retain_period_days">
    <rdfs:label>backup_retain_period_days</rdfs:label>
    <rdfs:comment>The period in days during which backups are stored.</rdfs:comment>
    <rdfs:domain rdf:resource="http://example.org/onto/class/yandex_mdb_clickhouse_cluster"/>
    <rdfs:range rdf:resource="http://www.w3.org/2001/XMLSchema#string"/>
  </owl:DatatypeProperty>
  <owl:DatatypeProperty rdf:about="http://example.org/onto/prop/yandex_mdb_clickhouse_cluster_cluster_id">
    <rdfs:label>cluster_id</rdfs:label>
    <rdfs:comment>The cluster identifier.</rdfs:comment>
    <rdfs:domain rdf:resource="http://example.org/onto/class/yandex_mdb_clickhouse_cluster"/>
    <rdfs:range rdf:resource="http://www.w3.org/2001/XMLSchema#string"/>
  </owl:DatatypeProperty>
  <owl:DatatypeProperty rdf:about="http://example.org/onto/prop/yandex_mdb_clickhouse_cluster_copy_schema_on_new_hosts">
    <rdfs:label>copy_schema_on_new_hosts</rdfs:label>
    <rdfs:comment>Whether to copy schema on new ClickHouse hosts.</rdfs:comment>
    <rdfs:domain rdf:resource="http://example.org/onto/class/yandex_mdb_clickhouse_cluster"/>
    <rdfs:range rdf:resource="http://www.w3.org/2001/XMLSchema#string"/>
  </owl:DatatypeProperty>
  <owl:DatatypeProperty rdf:about="http://example.org/onto/prop/yandex_mdb_clickhouse_cluster_created_at">
    <rdfs:label>created_at</rdfs:label>
    <rdfs:comment>The creation timestamp of the resource.</rdfs:comment>
    <rdfs:domain rdf:resource="http://example.org/onto/class/yandex_mdb_clickhouse_cluster"/>
    <rdfs:range rdf:resource="http://www.w3.org/2001/XMLSchema#string"/>
  </owl:DatatypeProperty>
  <owl:DatatypeProperty rdf:about="http://example.org/onto/prop/yandex_mdb_clickhouse_cluster_deletion_protection">
    <rdfs:label>deletion_protection</rdfs:label>
    <rdfs:comment>The `true` value means that resource is protected from accidental deletion.</rdfs:comment>
    <rdfs:domain rdf:resource="http://example.org/onto/class/yandex_mdb_clickhouse_cluster"/>
    <rdfs:range rdf:resource="http://www.w3.org/2001/XMLSchema#string"/>
  </owl:DatatypeProperty>
  <owl:DatatypeProperty rdf:about="http://example.org/onto/prop/yandex_mdb_clickhouse_cluster_description">
    <rdfs:label>description</rdfs:label>
    <rdfs:comment>The resource description.</rdfs:comment>
    <rdfs:domain rdf:resource="http://example.org/onto/class/yandex_mdb_clickhouse_cluster"/>
    <rdfs:range rdf:resource="http://www.w3.org/2001/XMLSchema#string"/>
  </owl:DatatypeProperty>
  <owl:DatatypeProperty rdf:about="http://example.org/onto/prop/yandex_mdb_clickhouse_cluster_disk_encryption_key_id">
    <rdfs:label>disk_encryption_key_id</rdfs:label>
    <rdfs:comment>ID of the KMS key for cluster disk encryption.</rdfs:comment>
    <rdfs:domain rdf:resource="http://example.org/onto/class/yandex_mdb_clickhouse_cluster"/>
    <rdfs:range rdf:resource="http://www.w3.org/2001/XMLSchema#string"/>
  </owl:DatatypeProperty>
  <owl:DatatypeProperty rdf:about="http://example.org/onto/prop/yandex_mdb_clickhouse_cluster_embedded_keeper">
    <rdfs:label>embedded_keeper</rdfs:label>
    <rdfs:comment>Whether to use ClickHouse Keeper as a coordination system and place it on the same hosts with ClickHouse. If not, it's used ZooKeeper with placement on separate hosts.</rdfs:comment>
    <rdfs:domain rdf:resource="http://example.org/onto/class/yandex_mdb_clickhouse_cluster"/>
    <rdfs:range rdf:resource="http://www.w3.org/2001/XMLSchema#string"/>
  </owl:DatatypeProperty>
  <owl:DatatypeProperty rdf:about="http://example.org/onto/prop/yandex_mdb_clickhouse_cluster_environment">
    <rdfs:label>environment</rdfs:label>
    <rdfs:comment>Deployment environment of the ClickHouse cluster. Can be either `PRESTABLE` or `PRODUCTION`.</rdfs:comment>
    <rdfs:domain rdf:resource="http://example.org/onto/class/yandex_mdb_clickhouse_cluster"/>
    <rdfs:range rdf:resource="http://www.w3.org/2001/XMLSchema#string"/>
  </owl:DatatypeProperty>
  <owl:DatatypeProperty rdf:about="http://example.org/onto/prop/yandex_mdb_clickhouse_cluster_folder_id">
    <rdfs:label>folder_id</rdfs:label>
    <rdfs:comment>The folder identifier that resource belongs to. If it is not provided, the default provider `folder-id` is used.</rdfs:comment>
    <rdfs:domain rdf:resource="http://example.org/onto/class/yandex_mdb_clickhouse_cluster"/>
    <rdfs:range rdf:resource="http://www.w3.org/2001/XMLSchema#string"/>
  </owl:DatatypeProperty>
  <owl:DatatypeProperty rdf:about="http://example.org/onto/prop/yandex_mdb_clickhouse_cluster_health">
    <rdfs:label>health</rdfs:label>
    <rdfs:comment>Aggregated health of the cluster. Can be `ALIVE`, `DEGRADED`, `DEAD` or `HEALTH_UNKNOWN`. For more information see `health` field of JSON representation in [the official documentation](https://yandex.cloud/docs/managed-clickhouse/api-ref/Cluster/).</rdfs:comment>
    <rdfs:domain rdf:resource="http://example.org/onto/class/yandex_mdb_clickhouse_cluster"/>
    <rdfs:range rdf:resource="http://www.w3.org/2001/XMLSchema#string"/>
  </owl:DatatypeProperty>
  <owl:DatatypeProperty rdf:about="http://example.org/onto/prop/yandex_mdb_clickhouse_cluster_id">
    <rdfs:label>id</rdfs:label>
    <rdfs:domain rdf:resource="http://example.org/onto/class/yandex_mdb_clickhouse_cluster"/>
    <rdfs:range rdf:resource="http://www.w3.org/2001/XMLSchema#string"/>
  </owl:DatatypeProperty>
  <owl:DatatypeProperty rdf:about="http://example.org/onto/prop/yandex_mdb_clickhouse_cluster_labels">
    <rdfs:label>labels</rdfs:label>
    <rdfs:comment>A set of key/value label pairs which assigned to resource.</rdfs:comment>
    <rdfs:domain rdf:resource="http://example.org/onto/class/yandex_mdb_clickhouse_cluster"/>
    <rdfs:range rdf:resource="http://www.w3.org/2001/XMLSchema#string"/>
  </owl:DatatypeProperty>
  <owl:DatatypeProperty rdf:about="http://example.org/onto/prop/yandex_mdb_clickhouse_cluster_name">
    <rdfs:label>name</rdfs:label>
    <rdfs:comment>The resource name.</rdfs:comment>
    <rdfs:domain rdf:resource="http://example.org/onto/class/yandex_mdb_clickhouse_cluster"/>
    <rdfs:range rdf:resource="http://www.w3.org/2001/XMLSchema#string"/>
  </owl:DatatypeProperty>
  <owl:DatatypeProperty rdf:about="http://example.org/onto/prop/yandex_mdb_clickhouse_cluster_network_id">
    <rdfs:label>network_id</rdfs:label>
    <rdfs:comment>The `VPC Network ID` of subnets which resource attached to.</rdfs:comment>
    <rdfs:domain rdf:resource="http://example.org/onto/class/yandex_mdb_clickhouse_cluster"/>
    <rdfs:range rdf:resource="http://www.w3.org/2001/XMLSchema#string"/>
  </owl:DatatypeProperty>
  <owl:DatatypeProperty rdf:about="http://example.org/onto/prop/yandex_mdb_clickhouse_cluster_security_group_ids">
    <rdfs:label>security_group_ids</rdfs:label>
    <rdfs:comment>The list of security groups applied to resource or their components.</rdfs:comment>
    <rdfs:domain rdf:resource="http://example.org/onto/class/yandex_mdb_clickhouse_cluster"/>
    <rdfs:range rdf:resource="http://www.w3.org/2001/XMLSchema#string"/>
  </owl:DatatypeProperty>
  <owl:DatatypeProperty rdf:about="http://example.org/onto/prop/yandex_mdb_clickhouse_cluster_service_account_id">
    <rdfs:label>service_account_id</rdfs:label>
    <rdfs:comment>[Service account](https://yandex.cloud/docs/iam/concepts/users/service-accounts) which linked to the resource.</rdfs:comment>
    <rdfs:domain rdf:resource="http://example.org/onto/class/yandex_mdb_clickhouse_cluster"/>
    <rdfs:range rdf:resource="http://www.w3.org/2001/XMLSchema#string"/>
  </owl:DatatypeProperty>
  <owl:DatatypeProperty rdf:about="http://example.org/onto/prop/yandex_mdb_clickhouse_cluster_sql_database_management">
    <rdfs:label>sql_database_management</rdfs:label>
    <rdfs:comment>Grants `admin` user database management permission.</rdfs:comment>
    <rdfs:domain rdf:resource="http://example.org/onto/class/yandex_mdb_clickhouse_cluster"/>
    <rdfs:range rdf:resource="http://www.w3.org/2001/XMLSchema#string"/>
  </owl:DatatypeProperty>
  <owl:DatatypeProperty rdf:about="http://example.org/onto/prop/yandex_mdb_clickhouse_cluster_sql_user_management">
    <rdfs:label>sql_user_management</rdfs:label>
    <rdfs:comment>Enables `admin` user with user management permission.</rdfs:comment>
    <rdfs:domain rdf:resource="http://example.org/onto/class/yandex_mdb_clickhouse_cluster"/>
    <rdfs:range rdf:resource="http://www.w3.org/2001/XMLSchema#string"/>
  </owl:DatatypeProperty>
  <owl:DatatypeProperty rdf:about="http://example.org/onto/prop/yandex_mdb_clickhouse_cluster_status">
    <rdfs:label>status</rdfs:label>
    <rdfs:comment>Status of the cluster. Can be `CREATING`, `STARTING`, `RUNNING`, `UPDATING`, `STOPPING`, `STOPPED`, `ERROR` or `STATUS_UNKNOWN`. For more information see `status` field of JSON representation in [the official documentation](https://yandex.cloud/docs/managed-clickhouse/api-ref/Cluster/).</rdfs:comment>
    <rdfs:domain rdf:resource="http://example.org/onto/class/yandex_mdb_clickhouse_cluster"/>
    <rdfs:range rdf:resource="http://www.w3.org/2001/XMLSchema#string"/>
  </owl:DatatypeProperty>
  <owl:DatatypeProperty rdf:about="http://example.org/onto/prop/yandex_mdb_clickhouse_cluster_version">
    <rdfs:label>version</rdfs:label>
    <rdfs:comment>Version of the ClickHouse server software.</rdfs:comment>
    <rdfs:domain rdf:resource="http://example.org/onto/class/yandex_mdb_clickhouse_cluster"/>
    <rdfs:range rdf:resource="http://www.w3.org/2001/XMLSchema#string"/>
  </owl:DatatypeProperty>
  <owl:DatatypeProperty rdf:about="http://example.org/onto/prop/yandex_mdb_clickhouse_cluster_data_lens">
    <rdfs:label>data_lens</rdfs:label>
    <rdfs:comment>Allow access for DataLens.</rdfs:comment>
    <rdfs:domain rdf:resource="http://example.org/onto/class/yandex_mdb_clickhouse_cluster"/>
    <rdfs:range rdf:resource="http://www.w3.org/2001/XMLSchema#string"/>
  </owl:DatatypeProperty>
  <owl:DatatypeProperty rdf:about="http://example.org/onto/prop/yandex_mdb_clickhouse_cluster_data_transfer">
    <rdfs:label>data_transfer</rdfs:label>
    <rdfs:comment>Allow access for DataTransfer.</rdfs:comment>
    <rdfs:domain rdf:resource="http://example.org/onto/class/yandex_mdb_clickhouse_cluster"/>
    <rdfs:range rdf:resource="http://www.w3.org/2001/XMLSchema#string"/>
  </owl:DatatypeProperty>
  <owl:DatatypeProperty rdf:about="http://example.org/onto/prop/yandex_mdb_clickhouse_cluster_metrika">
    <rdfs:label>metrika</rdfs:label>
    <rdfs:comment>Allow access for Yandex.Metrika.</rdfs:comment>
    <rdfs:domain rdf:resource="http://example.org/onto/class/yandex_mdb_clickhouse_cluster"/>
    <rdfs:range rdf:resource="http://www.w3.org/2001/XMLSchema#string"/>
  </owl:DatatypeProperty>
  <owl:DatatypeProperty rdf:about="http://example.org/onto/prop/yandex_mdb_clickhouse_cluster_serverless">
    <rdfs:label>serverless</rdfs:label>
    <rdfs:comment>Allow access for Serverless.</rdfs:comment>
    <rdfs:domain rdf:resource="http://example.org/onto/class/yandex_mdb_clickhouse_cluster"/>
    <rdfs:range rdf:resource="http://www.w3.org/2001/XMLSchema#string"/>
  </owl:DatatypeProperty>
  <owl:DatatypeProperty rdf:about="http://example.org/onto/prop/yandex_mdb_clickhouse_cluster_web_sql">
    <rdfs:label>web_sql</rdfs:label>
    <rdfs:comment>Allow access for Web SQL.</rdfs:comment>
    <rdfs:domain rdf:resource="http://example.org/onto/class/yandex_mdb_clickhouse_cluster"/>
    <rdfs:range rdf:resource="http://www.w3.org/2001/XMLSchema#string"/>
  </owl:DatatypeProperty>
  <owl:DatatypeProperty rdf:about="http://example.org/onto/prop/yandex_mdb_clickhouse_cluster_yandex_query">
    <rdfs:label>yandex_query</rdfs:label>
    <rdfs:comment>Allow access for YandexQuery.</rdfs:comment>
    <rdfs:domain rdf:resource="http://example.org/onto/class/yandex_mdb_clickhouse_cluster"/>
    <rdfs:range rdf:resource="http://www.w3.org/2001/XMLSchema#string"/>
  </owl:DatatypeProperty>
  <owl:DatatypeProperty rdf:about="http://example.org/onto/prop/yandex_mdb_clickhouse_cluster_hours">
    <rdfs:label>hours</rdfs:label>
    <rdfs:comment>The hour at which backup will be started.</rdfs:comment>
    <rdfs:domain rdf:resource="http://example.org/onto/class/yandex_mdb_clickhouse_cluster"/>
    <rdfs:range rdf:resource="http://www.w3.org/2001/XMLSchema#string"/>
  </owl:DatatypeProperty>
  <owl:DatatypeProperty rdf:about="http://example.org/onto/prop/yandex_mdb_clickhouse_cluster_minutes">
    <rdfs:label>minutes</rdfs:label>
    <rdfs:comment>The minute at which backup will be started.</rdfs:comment>
    <rdfs:domain rdf:resource="http://example.org/onto/class/yandex_mdb_clickhouse_cluster"/>
    <rdfs:range rdf:resource="http://www.w3.org/2001/XMLSchema#string"/>
  </owl:DatatypeProperty>
  <owl:DatatypeProperty rdf:about="http://example.org/onto/prop/yandex_mdb_clickhouse_cluster_asynchronous_insert_log_enabled">
    <rdfs:label>asynchronous_insert_log_enabled</rdfs:label>
    <rdfs:comment>Enable or disable asynchronous_insert_log system table.</rdfs:comment>
    <rdfs:domain rdf:resource="http://example.org/onto/class/yandex_mdb_clickhouse_cluster"/>
    <rdfs:range rdf:resource="http://www.w3.org/2001/XMLSchema#string"/>
  </owl:DatatypeProperty>
  <owl:DatatypeProperty rdf:about="http://example.org/onto/prop/yandex_mdb_clickhouse_cluster_asynchronous_insert_log_retention_size">
    <rdfs:label>asynchronous_insert_log_retention_size</rdfs:label>
    <rdfs:comment>The maximum size that asynchronous_insert_log can grow to before old data will be removed.</rdfs:comment>
    <rdfs:domain rdf:resource="http://example.org/onto/class/yandex_mdb_clickhouse_cluster"/>
    <rdfs:range rdf:resource="http://www.w3.org/2001/XMLSchema#string"/>
  </owl:DatatypeProperty>
  <owl:DatatypeProperty rdf:about="http://example.org/onto/prop/yandex_mdb_clickhouse_cluster_asynchronous_insert_log_retention_time">
    <rdfs:label>asynchronous_insert_log_retention_time</rdfs:label>
    <rdfs:comment>The maximum time that asynchronous_insert_log records will be retained before removal.</rdfs:comment>
    <rdfs:domain rdf:resource="http://example.org/onto/class/yandex_mdb_clickhouse_cluster"/>
    <rdfs:range rdf:resource="http://www.w3.org/2001/XMLSchema#string"/>
  </owl:DatatypeProperty>
  <owl:DatatypeProperty rdf:about="http://example.org/onto/prop/yandex_mdb_clickhouse_cluster_asynchronous_metric_log_enabled">
    <rdfs:label>asynchronous_metric_log_enabled</rdfs:label>
    <rdfs:comment>Enable or disable asynchronous_metric_log system table.</rdfs:comment>
    <rdfs:domain rdf:resource="http://example.org/onto/class/yandex_mdb_clickhouse_cluster"/>
    <rdfs:range rdf:resource="http://www.w3.org/2001/XMLSchema#string"/>
  </owl:DatatypeProperty>
  <owl:DatatypeProperty rdf:about="http://example.org/onto/prop/yandex_mdb_clickhouse_cluster_asynchronous_metric_log_retention_size">
    <rdfs:label>asynchronous_metric_log_retention_size</rdfs:label>
    <rdfs:comment>The maximum size that asynchronous_metric_log can grow to before old data will be removed.</rdfs:comment>
    <rdfs:domain rdf:resource="http://example.org/onto/class/yandex_mdb_clickhouse_cluster"/>
    <rdfs:range rdf:resource="http://www.w3.org/2001/XMLSchema#string"/>
  </owl:DatatypeProperty>
  <owl:DatatypeProperty rdf:about="http://example.org/onto/prop/yandex_mdb_clickhouse_cluster_asynchronous_metric_log_retention_time">
    <rdfs:label>asynchronous_metric_log_retention_time</rdfs:label>
    <rdfs:comment>The maximum time that asynchronous_metric_log records will be retained before removal.</rdfs:comment>
    <rdfs:domain rdf:resource="http://example.org/onto/class/yandex_mdb_clickhouse_cluster"/>
    <rdfs:range rdf:resource="http://www.w3.org/2001/XMLSchema#string"/>
  </owl:DatatypeProperty>
  <owl:DatatypeProperty rdf:about="http://example.org/onto/prop/yandex_mdb_clickhouse_cluster_background_buffer_flush_schedule_pool_size">
    <rdfs:label>background_buffer_flush_schedule_pool_size</rdfs:label>
    <rdfs:comment>The maximum number of threads that will be used for performing flush operations for Buffer-engine tables in the background.</rdfs:comment>
    <rdfs:domain rdf:resource="http://example.org/onto/class/yandex_mdb_clickhouse_cluster"/>
    <rdfs:range rdf:resource="http://www.w3.org/2001/XMLSchema#string"/>
  </owl:DatatypeProperty>
  <owl:DatatypeProperty rdf:about="http://example.org/onto/prop/yandex_mdb_clickhouse_cluster_background_common_pool_size">
    <rdfs:label>background_common_pool_size</rdfs:label>
    <rdfs:comment>The maximum number of threads that will be used for performing a variety of operations (mostly garbage collection) for MergeTree-engine tables in a background.</rdfs:comment>
    <rdfs:domain rdf:resource="http://example.org/onto/class/yandex_mdb_clickhouse_cluster"/>
    <rdfs:range rdf:resource="http://www.w3.org/2001/XMLSchema#string"/>
  </owl:DatatypeProperty>
  <owl:DatatypeProperty rdf:about="http://example.org/onto/prop/yandex_mdb_clickhouse_cluster_background_distributed_schedule_pool_size">
    <rdfs:label>background_distributed_schedule_pool_size</rdfs:label>
    <rdfs:comment>The maximum number of threads that will be used for executing distributed sends.</rdfs:comment>
    <rdfs:domain rdf:resource="http://example.org/onto/class/yandex_mdb_clickhouse_cluster"/>
    <rdfs:range rdf:resource="http://www.w3.org/2001/XMLSchema#string"/>
  </owl:DatatypeProperty>
  <owl:DatatypeProperty rdf:about="http://example.org/onto/prop/yandex_mdb_clickhouse_cluster_background_fetches_pool_size">
    <rdfs:label>background_fetches_pool_size</rdfs:label>
    <rdfs:comment>The maximum number of threads that will be used for fetching data parts from another replica for MergeTree-engine tables in a background.</rdfs:comment>
    <rdfs:domain rdf:resource="http://example.org/onto/class/yandex_mdb_clickhouse_cluster"/>
    <rdfs:range rdf:resource="http://www.w3.org/2001/XMLSchema#string"/>
  </owl:DatatypeProperty>
  <owl:DatatypeProperty rdf:about="http://example.org/onto/prop/yandex_mdb_clickhouse_cluster_background_merges_mutations_concurrency_ratio">
    <rdfs:label>background_merges_mutations_concurrency_ratio</rdfs:label>
    <rdfs:comment>Sets a ratio between the number of threads and the number of background merges and mutations that can be executed concurrently.</rdfs:comment>
    <rdfs:domain rdf:resource="http://example.org/onto/class/yandex_mdb_clickhouse_cluster"/>
    <rdfs:range rdf:resource="http://www.w3.org/2001/XMLSchema#string"/>
  </owl:DatatypeProperty>
  <owl:DatatypeProperty rdf:about="http://example.org/onto/prop/yandex_mdb_clickhouse_cluster_background_message_broker_schedule_pool_size">
    <rdfs:label>background_message_broker_schedule_pool_size</rdfs:label>
    <rdfs:comment>The maximum number of threads that will be used for executing background operations for message streaming.</rdfs:comment>
    <rdfs:domain rdf:resource="http://example.org/onto/class/yandex_mdb_clickhouse_cluster"/>
    <rdfs:range rdf:resource="http://www.w3.org/2001/XMLSchema#string"/>
  </owl:DatatypeProperty>
  <owl:DatatypeProperty rdf:about="http://example.org/onto/prop/yandex_mdb_clickhouse_cluster_background_move_pool_size">
    <rdfs:label>background_move_pool_size</rdfs:label>
    <rdfs:comment>The maximum number of threads that will be used for moving data parts to another disk or volume for MergeTree-engine tables in a background.</rdfs:comment>
    <rdfs:domain rdf:resource="http://example.org/onto/class/yandex_mdb_clickhouse_cluster"/>
    <rdfs:range rdf:resource="http://www.w3.org/2001/XMLSchema#string"/>
  </owl:DatatypeProperty>
  <owl:DatatypeProperty rdf:about="http://example.org/onto/prop/yandex_mdb_clickhouse_cluster_background_pool_size">
    <rdfs:label>background_pool_size</rdfs:label>
    <rdfs:comment>Sets the number of threads performing background merges and mutations for MergeTree-engine tables.</rdfs:comment>
    <rdfs:domain rdf:resource="http://example.org/onto/class/yandex_mdb_clickhouse_cluster"/>
    <rdfs:range rdf:resource="http://www.w3.org/2001/XMLSchema#string"/>
  </owl:DatatypeProperty>
  <owl:DatatypeProperty rdf:about="http://example.org/onto/prop/yandex_mdb_clickhouse_cluster_background_schedule_pool_size">
    <rdfs:label>background_schedule_pool_size</rdfs:label>
    <rdfs:comment>The maximum number of threads that will be used for constantly executing some lightweight periodic operations for replicated tables, Kafka streaming, and DNS cache updates.</rdfs:comment>
    <rdfs:domain rdf:resource="http://example.org/onto/class/yandex_mdb_clickhouse_cluster"/>
    <rdfs:range rdf:resource="http://www.w3.org/2001/XMLSchema#string"/>
  </owl:DatatypeProperty>
  <owl:DatatypeProperty rdf:about="http://example.org/onto/prop/yandex_mdb_clickhouse_cluster_default_database">
    <rdfs:label>default_database</rdfs:label>
    <rdfs:comment>Default database name.</rdfs:comment>
    <rdfs:domain rdf:resource="http://example.org/onto/class/yandex_mdb_clickhouse_cluster"/>
    <rdfs:range rdf:resource="http://www.w3.org/2001/XMLSchema#string"/>
  </owl:DatatypeProperty>
  <owl:DatatypeProperty rdf:about="http://example.org/onto/prop/yandex_mdb_clickhouse_cluster_dictionaries_lazy_load">
    <rdfs:label>dictionaries_lazy_load</rdfs:label>
    <rdfs:comment>Lazy loading of dictionaries. If true, then each dictionary is loaded on the first use.</rdfs:comment>
    <rdfs:domain rdf:resource="http://example.org/onto/class/yandex_mdb_clickhouse_cluster"/>
    <rdfs:range rdf:resource="http://www.w3.org/2001/XMLSchema#string"/>
  </owl:DatatypeProperty>
  <owl:DatatypeProperty rdf:about="http://example.org/onto/prop/yandex_mdb_clickhouse_cluster_geobase_enabled">
    <rdfs:label>geobase_enabled</rdfs:label>
    <rdfs:comment>Enable or disable geobase.</rdfs:comment>
    <rdfs:domain rdf:resource="http://example.org/onto/class/yandex_mdb_clickhouse_cluster"/>
    <rdfs:range rdf:resource="http://www.w3.org/2001/XMLSchema#string"/>
  </owl:DatatypeProperty>
  <owl:DatatypeProperty rdf:about="http://example.org/onto/prop/yandex_mdb_clickhouse_cluster_geobase_uri">
    <rdfs:label>geobase_uri</rdfs:label>
    <rdfs:comment>Address of the archive with the user geobase in Object Storage.</rdfs:comment>
    <rdfs:domain rdf:resource="http://example.org/onto/class/yandex_mdb_clickhouse_cluster"/>
    <rdfs:range rdf:resource="http://www.w3.org/2001/XMLSchema#string"/>
  </owl:DatatypeProperty>
  <owl:DatatypeProperty rdf:about="http://example.org/onto/prop/yandex_mdb_clickhouse_cluster_keep_alive_timeout">
    <rdfs:label>keep_alive_timeout</rdfs:label>
    <rdfs:comment>The number of seconds that ClickHouse waits for incoming requests for HTTP protocol before closing the connection.</rdfs:comment>
    <rdfs:domain rdf:resource="http://example.org/onto/class/yandex_mdb_clickhouse_cluster"/>
    <rdfs:range rdf:resource="http://www.w3.org/2001/XMLSchema#string"/>
  </owl:DatatypeProperty>
  <owl:DatatypeProperty rdf:about="http://example.org/onto/prop/yandex_mdb_clickhouse_cluster_log_level">
    <rdfs:label>log_level</rdfs:label>
    <rdfs:comment>Logging level.</rdfs:comment>
    <rdfs:domain rdf:resource="http://example.org/onto/class/yandex_mdb_clickhouse_cluster"/>
    <rdfs:range rdf:resource="http://www.w3.org/2001/XMLSchema#string"/>
  </owl:DatatypeProperty>
  <owl:DatatypeProperty rdf:about="http://example.org/onto/prop/yandex_mdb_clickhouse_cluster_mark_cache_size">
    <rdfs:label>mark_cache_size</rdfs:label>
    <rdfs:comment>Maximum size of cache for marks</rdfs:comment>
    <rdfs:domain rdf:resource="http://example.org/onto/class/yandex_mdb_clickhouse_cluster"/>
    <rdfs:range rdf:resource="http://www.w3.org/2001/XMLSchema#string"/>
  </owl:DatatypeProperty>
  <owl:DatatypeProperty rdf:about="http://example.org/onto/prop/yandex_mdb_clickhouse_cluster_max_concurrent_queries">
    <rdfs:label>max_concurrent_queries</rdfs:label>
    <rdfs:comment>Limit on total number of concurrently executed queries.</rdfs:comment>
    <rdfs:domain rdf:resource="http://example.org/onto/class/yandex_mdb_clickhouse_cluster"/>
    <rdfs:range rdf:resource="http://www.w3.org/2001/XMLSchema#string"/>
  </owl:DatatypeProperty>
  <owl:DatatypeProperty rdf:about="http://example.org/onto/prop/yandex_mdb_clickhouse_cluster_max_connections">
    <rdfs:label>max_connections</rdfs:label>
    <rdfs:comment>Max server connections.</rdfs:comment>
    <rdfs:domain rdf:resource="http://example.org/onto/class/yandex_mdb_clickhouse_cluster"/>
    <rdfs:range rdf:resource="http://www.w3.org/2001/XMLSchema#string"/>
  </owl:DatatypeProperty>
  <owl:DatatypeProperty rdf:about="http://example.org/onto/prop/yandex_mdb_clickhouse_cluster_max_partition_size_to_drop">
    <rdfs:label>max_partition_size_to_drop</rdfs:label>
    <rdfs:comment>Restriction on dropping partitions.</rdfs:comment>
    <rdfs:domain rdf:resource="http://example.org/onto/class/yandex_mdb_clickhouse_cluster"/>
    <rdfs:range rdf:resource="http://www.w3.org/2001/XMLSchema#string"/>
  </owl:DatatypeProperty>
  <owl:DatatypeProperty rdf:about="http://example.org/onto/prop/yandex_mdb_clickhouse_cluster_max_table_size_to_drop">
    <rdfs:label>max_table_size_to_drop</rdfs:label>
    <rdfs:comment>Restriction on deleting tables.</rdfs:comment>
    <rdfs:domain rdf:resource="http://example.org/onto/class/yandex_mdb_clickhouse_cluster"/>
    <rdfs:range rdf:resource="http://www.w3.org/2001/XMLSchema#string"/>
  </owl:DatatypeProperty>
  <owl:DatatypeProperty rdf:about="http://example.org/onto/prop/yandex_mdb_clickhouse_cluster_metric_log_enabled">
    <rdfs:label>metric_log_enabled</rdfs:label>
    <rdfs:comment>Enable or disable metric_log system table.</rdfs:comment>
    <rdfs:domain rdf:resource="http://example.org/onto/class/yandex_mdb_clickhouse_cluster"/>
    <rdfs:range rdf:resource="http://www.w3.org/2001/XMLSchema#string"/>
  </owl:DatatypeProperty>
  <owl:DatatypeProperty rdf:about="http://example.org/onto/prop/yandex_mdb_clickhouse_cluster_metric_log_retention_size">
    <rdfs:label>metric_log_retention_size</rdfs:label>
    <rdfs:comment>The maximum size that metric_log can grow to before old data will be removed.</rdfs:comment>
    <rdfs:domain rdf:resource="http://example.org/onto/class/yandex_mdb_clickhouse_cluster"/>
    <rdfs:range rdf:resource="http://www.w3.org/2001/XMLSchema#string"/>
  </owl:DatatypeProperty>
  <owl:DatatypeProperty rdf:about="http://example.org/onto/prop/yandex_mdb_clickhouse_cluster_metric_log_retention_time">
    <rdfs:label>metric_log_retention_time</rdfs:label>
    <rdfs:comment>The maximum time that metric_log records will be retained before removal.</rdfs:comment>
    <rdfs:domain rdf:resource="http://example.org/onto/class/yandex_mdb_clickhouse_cluster"/>
    <rdfs:range rdf:resource="http://www.w3.org/2001/XMLSchema#string"/>
  </owl:DatatypeProperty>
  <owl:DatatypeProperty rdf:about="http://example.org/onto/prop/yandex_mdb_clickhouse_cluster_opentelemetry_span_log_enabled">
    <rdfs:label>opentelemetry_span_log_enabled</rdfs:label>
    <rdfs:comment>Enable or disable opentelemetry_span_log system table.</rdfs:comment>
    <rdfs:domain rdf:resource="http://example.org/onto/class/yandex_mdb_clickhouse_cluster"/>
    <rdfs:range rdf:resource="http://www.w3.org/2001/XMLSchema#string"/>
  </owl:DatatypeProperty>
  <owl:DatatypeProperty rdf:about="http://example.org/onto/prop/yandex_mdb_clickhouse_cluster_opentelemetry_span_log_retention_size">
    <rdfs:label>opentelemetry_span_log_retention_size</rdfs:label>
    <rdfs:comment>The maximum size that opentelemetry_span_log can grow to before old data will be removed.</rdfs:comment>
    <rdfs:domain rdf:resource="http://example.org/onto/class/yandex_mdb_clickhouse_cluster"/>
    <rdfs:range rdf:resource="http://www.w3.org/2001/XMLSchema#string"/>
  </owl:DatatypeProperty>
  <owl:DatatypeProperty rdf:about="http://example.org/onto/prop/yandex_mdb_clickhouse_cluster_opentelemetry_span_log_retention_time">
    <rdfs:label>opentelemetry_span_log_retention_time</rdfs:label>
    <rdfs:comment>The maximum time that opentelemetry_span_log records will be retained before removal.</rdfs:comment>
    <rdfs:domain rdf:resource="http://example.org/onto/class/yandex_mdb_clickhouse_cluster"/>
    <rdfs:range rdf:resource="http://www.w3.org/2001/XMLSchema#string"/>
  </owl:DatatypeProperty>
  <owl:DatatypeProperty rdf:about="http://example.org/onto/prop/yandex_mdb_clickhouse_cluster_part_log_retention_size">
    <rdfs:label>part_log_retention_size</rdfs:label>
    <rdfs:comment>The maximum size that part_log can grow to before old data will be removed.</rdfs:comment>
    <rdfs:domain rdf:resource="http://example.org/onto/class/yandex_mdb_clickhouse_cluster"/>
    <rdfs:range rdf:resource="http://www.w3.org/2001/XMLSchema#string"/>
  </owl:DatatypeProperty>
  <owl:DatatypeProperty rdf:about="http://example.org/onto/prop/yandex_mdb_clickhouse_cluster_part_log_retention_time">
    <rdfs:label>part_log_retention_time</rdfs:label>
    <rdfs:comment>The maximum time that part_log records will be retained before removal.</rdfs:comment>
    <rdfs:domain rdf:resource="http://example.org/onto/class/yandex_mdb_clickhouse_cluster"/>
    <rdfs:range rdf:resource="http://www.w3.org/2001/XMLSchema#string"/>
  </owl:DatatypeProperty>
  <owl:DatatypeProperty rdf:about="http://example.org/onto/prop/yandex_mdb_clickhouse_cluster_query_log_retention_size">
    <rdfs:label>query_log_retention_size</rdfs:label>
    <rdfs:comment>The maximum size that query_log can grow to before old data will be removed.</rdfs:comment>
    <rdfs:domain rdf:resource="http://example.org/onto/class/yandex_mdb_clickhouse_cluster"/>
    <rdfs:range rdf:resource="http://www.w3.org/2001/XMLSchema#string"/>
  </owl:DatatypeProperty>
  <owl:DatatypeProperty rdf:about="http://example.org/onto/prop/yandex_mdb_clickhouse_cluster_query_log_retention_time">
    <rdfs:label>query_log_retention_time</rdfs:label>
    <rdfs:comment>The maximum time that query_log records will be retained before removal.</rdfs:comment>
    <rdfs:domain rdf:resource="http://example.org/onto/class/yandex_mdb_clickhouse_cluster"/>
    <rdfs:range rdf:resource="http://www.w3.org/2001/XMLSchema#string"/>
  </owl:DatatypeProperty>
  <owl:DatatypeProperty rdf:about="http://example.org/onto/prop/yandex_mdb_clickhouse_cluster_query_thread_log_enabled">
    <rdfs:label>query_thread_log_enabled</rdfs:label>
    <rdfs:comment>Enable or disable query_thread_log system table.</rdfs:comment>
    <rdfs:domain rdf:resource="http://example.org/onto/class/yandex_mdb_clickhouse_cluster"/>
    <rdfs:range rdf:resource="http://www.w3.org/2001/XMLSchema#string"/>
  </owl:DatatypeProperty>
  <owl:DatatypeProperty rdf:about="http://example.org/onto/prop/yandex_mdb_clickhouse_cluster_query_thread_log_retention_size">
    <rdfs:label>query_thread_log_retention_size</rdfs:label>
    <rdfs:comment>The maximum size that query_thread_log can grow to before old data will be removed.</rdfs:comment>
    <rdfs:domain rdf:resource="http://example.org/onto/class/yandex_mdb_clickhouse_cluster"/>
    <rdfs:range rdf:resource="http://www.w3.org/2001/XMLSchema#string"/>
  </owl:DatatypeProperty>
  <owl:DatatypeProperty rdf:about="http://example.org/onto/prop/yandex_mdb_clickhouse_cluster_query_thread_log_retention_time">
    <rdfs:label>query_thread_log_retention_time</rdfs:label>
    <rdfs:comment>The maximum time that query_thread_log records will be retained before removal.</rdfs:comment>
    <rdfs:domain rdf:resource="http://example.org/onto/class/yandex_mdb_clickhouse_cluster"/>
    <rdfs:range rdf:resource="http://www.w3.org/2001/XMLSchema#string"/>
  </owl:DatatypeProperty>
  <owl:DatatypeProperty rdf:about="http://example.org/onto/prop/yandex_mdb_clickhouse_cluster_query_views_log_enabled">
    <rdfs:label>query_views_log_enabled</rdfs:label>
    <rdfs:comment>Enable or disable query_views_log system table.</rdfs:comment>
    <rdfs:domain rdf:resource="http://example.org/onto/class/yandex_mdb_clickhouse_cluster"/>
    <rdfs:range rdf:resource="http://www.w3.org/2001/XMLSchema#string"/>
  </owl:DatatypeProperty>
  <owl:DatatypeProperty rdf:about="http://example.org/onto/prop/yandex_mdb_clickhouse_cluster_query_views_log_retention_size">
    <rdfs:label>query_views_log_retention_size</rdfs:label>
    <rdfs:comment>The maximum size that query_views_log can grow to before old data will be removed.</rdfs:comment>
    <rdfs:domain rdf:resource="http://example.org/onto/class/yandex_mdb_clickhouse_cluster"/>
    <rdfs:range rdf:resource="http://www.w3.org/2001/XMLSchema#string"/>
  </owl:DatatypeProperty>
  <owl:DatatypeProperty rdf:about="http://example.org/onto/prop/yandex_mdb_clickhouse_cluster_query_views_log_retention_time">
    <rdfs:label>query_views_log_retention_time</rdfs:label>
    <rdfs:comment>The maximum time that query_views_log records will be retained before removal.</rdfs:comment>
    <rdfs:domain rdf:resource="http://example.org/onto/class/yandex_mdb_clickhouse_cluster"/>
    <rdfs:range rdf:resource="http://www.w3.org/2001/XMLSchema#string"/>
  </owl:DatatypeProperty>
  <owl:DatatypeProperty rdf:about="http://example.org/onto/prop/yandex_mdb_clickhouse_cluster_session_log_enabled">
    <rdfs:label>session_log_enabled</rdfs:label>
    <rdfs:comment>Enable or disable session_log system table.</rdfs:comment>
    <rdfs:domain rdf:resource="http://example.org/onto/class/yandex_mdb_clickhouse_cluster"/>
    <rdfs:range rdf:resource="http://www.w3.org/2001/XMLSchema#string"/>
  </owl:DatatypeProperty>
  <owl:DatatypeProperty rdf:about="http://example.org/onto/prop/yandex_mdb_clickhouse_cluster_session_log_retention_size">
    <rdfs:label>session_log_retention_size</rdfs:label>
    <rdfs:comment>The maximum size that session_log can grow to before old data will be removed.</rdfs:comment>
    <rdfs:domain rdf:resource="http://example.org/onto/class/yandex_mdb_clickhouse_cluster"/>
    <rdfs:range rdf:resource="http://www.w3.org/2001/XMLSchema#string"/>
  </owl:DatatypeProperty>
  <owl:DatatypeProperty rdf:about="http://example.org/onto/prop/yandex_mdb_clickhouse_cluster_session_log_retention_time">
    <rdfs:label>session_log_retention_time</rdfs:label>
    <rdfs:comment>The maximum time that session_log records will be retained before removal.</rdfs:comment>
    <rdfs:domain rdf:resource="http://example.org/onto/class/yandex_mdb_clickhouse_cluster"/>
    <rdfs:range rdf:resource="http://www.w3.org/2001/XMLSchema#string"/>
  </owl:DatatypeProperty>
  <owl:DatatypeProperty rdf:about="http://example.org/onto/prop/yandex_mdb_clickhouse_cluster_text_log_enabled">
    <rdfs:label>text_log_enabled</rdfs:label>
    <rdfs:comment>Enable or disable text_log system table.</rdfs:comment>
    <rdfs:domain rdf:resource="http://example.org/onto/class/yandex_mdb_clickhouse_cluster"/>
    <rdfs:range rdf:resource="http://www.w3.org/2001/XMLSchema#string"/>
  </owl:DatatypeProperty>
  <owl:DatatypeProperty rdf:about="http://example.org/onto/prop/yandex_mdb_clickhouse_cluster_text_log_level">
    <rdfs:label>text_log_level</rdfs:label>
    <rdfs:comment>Logging level for text_log system table.</rdfs:comment>
    <rdfs:domain rdf:resource="http://example.org/onto/class/yandex_mdb_clickhouse_cluster"/>
    <rdfs:range rdf:resource="http://www.w3.org/2001/XMLSchema#string"/>
  </owl:DatatypeProperty>
  <owl:DatatypeProperty rdf:about="http://example.org/onto/prop/yandex_mdb_clickhouse_cluster_text_log_retention_size">
    <rdfs:label>text_log_retention_size</rdfs:label>
    <rdfs:comment>The maximum size that text_log can grow to before old data will be removed.</rdfs:comment>
    <rdfs:domain rdf:resource="http://example.org/onto/class/yandex_mdb_clickhouse_cluster"/>
    <rdfs:range rdf:resource="http://www.w3.org/2001/XMLSchema#string"/>
  </owl:DatatypeProperty>
  <owl:DatatypeProperty rdf:about="http://example.org/onto/prop/yandex_mdb_clickhouse_cluster_text_log_retention_time">
    <rdfs:label>text_log_retention_time</rdfs:label>
    <rdfs:comment>The maximum time that text_log records will be retained before removal.</rdfs:comment>
    <rdfs:domain rdf:resource="http://example.org/onto/class/yandex_mdb_clickhouse_cluster"/>
    <rdfs:range rdf:resource="http://www.w3.org/2001/XMLSchema#string"/>
  </owl:DatatypeProperty>
  <owl:DatatypeProperty rdf:about="http://example.org/onto/prop/yandex_mdb_clickhouse_cluster_timezone">
    <rdfs:label>timezone</rdfs:label>
    <rdfs:comment>The server's time zone.</rdfs:comment>
    <rdfs:domain rdf:resource="http://example.org/onto/class/yandex_mdb_clickhouse_cluster"/>
    <rdfs:range rdf:resource="http://www.w3.org/2001/XMLSchema#string"/>
  </owl:DatatypeProperty>
  <owl:DatatypeProperty rdf:about="http://example.org/onto/prop/yandex_mdb_clickhouse_cluster_total_memory_profiler_step">
    <rdfs:label>total_memory_profiler_step</rdfs:label>
    <rdfs:comment>Whenever server memory usage becomes larger than every next step in number of bytes the memory profiler will collect the allocating stack trace.</rdfs:comment>
    <rdfs:domain rdf:resource="http://example.org/onto/class/yandex_mdb_clickhouse_cluster"/>
    <rdfs:range rdf:resource="http://www.w3.org/2001/XMLSchema#string"/>
  </owl:DatatypeProperty>
  <owl:DatatypeProperty rdf:about="http://example.org/onto/prop/yandex_mdb_clickhouse_cluster_trace_log_enabled">
    <rdfs:label>trace_log_enabled</rdfs:label>
    <rdfs:comment>Enable or disable trace_log system table.</rdfs:comment>
    <rdfs:domain rdf:resource="http://example.org/onto/class/yandex_mdb_clickhouse_cluster"/>
    <rdfs:range rdf:resource="http://www.w3.org/2001/XMLSchema#string"/>
  </owl:DatatypeProperty>
  <owl:DatatypeProperty rdf:about="http://example.org/onto/prop/yandex_mdb_clickhouse_cluster_trace_log_retention_size">
    <rdfs:label>trace_log_retention_size</rdfs:label>
    <rdfs:comment>The maximum size that trace_log can grow to before old data will be removed.</rdfs:comment>
    <rdfs:domain rdf:resource="http://example.org/onto/class/yandex_mdb_clickhouse_cluster"/>
    <rdfs:range rdf:resource="http://www.w3.org/2001/XMLSchema#string"/>
  </owl:DatatypeProperty>
  <owl:DatatypeProperty rdf:about="http://example.org/onto/prop/yandex_mdb_clickhouse_cluster_trace_log_retention_time">
    <rdfs:label>trace_log_retention_time</rdfs:label>
    <rdfs:comment>The maximum time that trace_log records will be retained before removal.</rdfs:comment>
    <rdfs:domain rdf:resource="http://example.org/onto/class/yandex_mdb_clickhouse_cluster"/>
    <rdfs:range rdf:resource="http://www.w3.org/2001/XMLSchema#string"/>
  </owl:DatatypeProperty>
  <owl:DatatypeProperty rdf:about="http://example.org/onto/prop/yandex_mdb_clickhouse_cluster_uncompressed_cache_size">
    <rdfs:label>uncompressed_cache_size</rdfs:label>
    <rdfs:comment>Cache size (in bytes) for uncompressed data used by table engines from the MergeTree family. Zero means disabled.</rdfs:comment>
    <rdfs:domain rdf:resource="http://example.org/onto/class/yandex_mdb_clickhouse_cluster"/>
    <rdfs:range rdf:resource="http://www.w3.org/2001/XMLSchema#string"/>
  </owl:DatatypeProperty>
  <owl:DatatypeProperty rdf:about="http://example.org/onto/prop/yandex_mdb_clickhouse_cluster_zookeeper_log_enabled">
    <rdfs:label>zookeeper_log_enabled</rdfs:label>
    <rdfs:comment>Enable or disable zookeeper_log system table.</rdfs:comment>
    <rdfs:domain rdf:resource="http://example.org/onto/class/yandex_mdb_clickhouse_cluster"/>
    <rdfs:range rdf:resource="http://www.w3.org/2001/XMLSchema#string"/>
  </owl:DatatypeProperty>
  <owl:DatatypeProperty rdf:about="http://example.org/onto/prop/yandex_mdb_clickhouse_cluster_zookeeper_log_retention_size">
    <rdfs:label>zookeeper_log_retention_size</rdfs:label>
    <rdfs:comment>The maximum size that zookeeper_log can grow to before old data will be removed.</rdfs:comment>
    <rdfs:domain rdf:resource="http://example.org/onto/class/yandex_mdb_clickhouse_cluster"/>
    <rdfs:range rdf:resource="http://www.w3.org/2001/XMLSchema#string"/>
  </owl:DatatypeProperty>
  <owl:DatatypeProperty rdf:about="http://example.org/onto/prop/yandex_mdb_clickhouse_cluster_zookeeper_log_retention_time">
    <rdfs:label>zookeeper_log_retention_time</rdfs:label>
    <rdfs:comment>The maximum time that zookeeper_log records will be retained before removal.</rdfs:comment>
    <rdfs:domain rdf:resource="http://example.org/onto/class/yandex_mdb_clickhouse_cluster"/>
    <rdfs:range rdf:resource="http://www.w3.org/2001/XMLSchema#string"/>
  </owl:DatatypeProperty>
  <owl:DatatypeProperty rdf:about="http://example.org/onto/prop/yandex_mdb_clickhouse_cluster_level">
    <rdfs:label>level</rdfs:label>
    <rdfs:comment>Compression level for `ZSTD` method.</rdfs:comment>
    <rdfs:domain rdf:resource="http://example.org/onto/class/yandex_mdb_clickhouse_cluster"/>
    <rdfs:range rdf:resource="http://www.w3.org/2001/XMLSchema#string"/>
  </owl:DatatypeProperty>
  <owl:DatatypeProperty rdf:about="http://example.org/onto/prop/yandex_mdb_clickhouse_cluster_method">
    <rdfs:label>method</rdfs:label>
    <rdfs:comment>Compression method. Two methods are available: `LZ4` and `zstd`.</rdfs:comment>
    <rdfs:domain rdf:resource="http://example.org/onto/class/yandex_mdb_clickhouse_cluster"/>
    <rdfs:range rdf:resource="http://www.w3.org/2001/XMLSchema#string"/>
  </owl:DatatypeProperty>
  <owl:DatatypeProperty rdf:about="http://example.org/onto/prop/yandex_mdb_clickhouse_cluster_min_part_size">
    <rdfs:label>min_part_size</rdfs:label>
    <rdfs:comment>Min part size: Minimum size (in bytes) of a data part in a table. ClickHouse only applies the rule to tables with data parts greater than or equal to the Min part size value.</rdfs:comment>
    <rdfs:domain rdf:resource="http://example.org/onto/class/yandex_mdb_clickhouse_cluster"/>
    <rdfs:range rdf:resource="http://www.w3.org/2001/XMLSchema#string"/>
  </owl:DatatypeProperty>
  <owl:DatatypeProperty rdf:about="http://example.org/onto/prop/yandex_mdb_clickhouse_cluster_min_part_size_ratio">
    <rdfs:label>min_part_size_ratio</rdfs:label>
    <rdfs:comment>Min part size ratio: Minimum table part size to total table size ratio. ClickHouse only applies the rule to tables in which this ratio is greater than or equal to the Min part size ratio value.</rdfs:comment>
    <rdfs:domain rdf:resource="http://example.org/onto/class/yandex_mdb_clickhouse_cluster"/>
    <rdfs:range rdf:resource="http://www.w3.org/2001/XMLSchema#string"/>
  </owl:DatatypeProperty>
  <owl:DatatypeProperty rdf:about="http://example.org/onto/prop/yandex_mdb_clickhouse_cluster_name">
    <rdfs:label>name</rdfs:label>
    <rdfs:comment>Graphite rollup configuration name.</rdfs:comment>
    <rdfs:domain rdf:resource="http://example.org/onto/class/yandex_mdb_clickhouse_cluster"/>
    <rdfs:range rdf:resource="http://www.w3.org/2001/XMLSchema#string"/>
  </owl:DatatypeProperty>
  <owl:DatatypeProperty rdf:about="http://example.org/onto/prop/yandex_mdb_clickhouse_cluster_path_column_name">
    <rdfs:label>path_column_name</rdfs:label>
    <rdfs:comment>The name of the column storing the metric name (Graphite sensor). Default value: Path.</rdfs:comment>
    <rdfs:domain rdf:resource="http://example.org/onto/class/yandex_mdb_clickhouse_cluster"/>
    <rdfs:range rdf:resource="http://www.w3.org/2001/XMLSchema#string"/>
  </owl:DatatypeProperty>
  <owl:DatatypeProperty rdf:about="http://example.org/onto/prop/yandex_mdb_clickhouse_cluster_time_column_name">
    <rdfs:label>time_column_name</rdfs:label>
    <rdfs:comment>The name of the column storing the time of measuring the metric. Default value: Time.</rdfs:comment>
    <rdfs:domain rdf:resource="http://example.org/onto/class/yandex_mdb_clickhouse_cluster"/>
    <rdfs:range rdf:resource="http://www.w3.org/2001/XMLSchema#string"/>
  </owl:DatatypeProperty>
  <owl:DatatypeProperty rdf:about="http://example.org/onto/prop/yandex_mdb_clickhouse_cluster_value_column_name">
    <rdfs:label>value_column_name</rdfs:label>
    <rdfs:comment>The name of the column storing the value of the metric at the time set in `time_column_name`. Default value: Value.</rdfs:comment>
    <rdfs:domain rdf:resource="http://example.org/onto/class/yandex_mdb_clickhouse_cluster"/>
    <rdfs:range rdf:resource="http://www.w3.org/2001/XMLSchema#string"/>
  </owl:DatatypeProperty>
  <owl:DatatypeProperty rdf:about="http://example.org/onto/prop/yandex_mdb_clickhouse_cluster_version_column_name">
    <rdfs:label>version_column_name</rdfs:label>
    <rdfs:comment>The name of the column storing the version of the metric. Default value: Timestamp.</rdfs:comment>
    <rdfs:domain rdf:resource="http://example.org/onto/class/yandex_mdb_clickhouse_cluster"/>
    <rdfs:range rdf:resource="http://www.w3.org/2001/XMLSchema#string"/>
  </owl:DatatypeProperty>
  <owl:DatatypeProperty rdf:about="http://example.org/onto/prop/yandex_mdb_clickhouse_cluster_function">
    <rdfs:label>function</rdfs:label>
    <rdfs:comment>Aggregation function name.</rdfs:comment>
    <rdfs:domain rdf:resource="http://example.org/onto/class/yandex_mdb_clickhouse_cluster"/>
    <rdfs:range rdf:resource="http://www.w3.org/2001/XMLSchema#string"/>
  </owl:DatatypeProperty>
  <owl:DatatypeProperty rdf:about="http://example.org/onto/prop/yandex_mdb_clickhouse_cluster_regexp">
    <rdfs:label>regexp</rdfs:label>
    <rdfs:comment>Regular expression that the metric name must match.</rdfs:comment>
    <rdfs:domain rdf:resource="http://example.org/onto/class/yandex_mdb_clickhouse_cluster"/>
    <rdfs:range rdf:resource="http://www.w3.org/2001/XMLSchema#string"/>
  </owl:DatatypeProperty>
  <owl:DatatypeProperty rdf:about="http://example.org/onto/prop/yandex_mdb_clickhouse_cluster_age">
    <rdfs:label>age</rdfs:label>
    <rdfs:comment>Minimum data age in seconds.</rdfs:comment>
    <rdfs:domain rdf:resource="http://example.org/onto/class/yandex_mdb_clickhouse_cluster"/>
    <rdfs:range rdf:resource="http://www.w3.org/2001/XMLSchema#string"/>
  </owl:DatatypeProperty>
  <owl:DatatypeProperty rdf:about="http://example.org/onto/prop/yandex_mdb_clickhouse_cluster_precision">
    <rdfs:label>precision</rdfs:label>
    <rdfs:comment>Accuracy of determining the age of the data in seconds.</rdfs:comment>
    <rdfs:domain rdf:resource="http://example.org/onto/class/yandex_mdb_clickhouse_cluster"/>
    <rdfs:range rdf:resource="http://www.w3.org/2001/XMLSchema#string"/>
  </owl:DatatypeProperty>
  <owl:DatatypeProperty rdf:about="http://example.org/onto/prop/yandex_mdb_clickhouse_cluster_host">
    <rdfs:label>host</rdfs:label>
    <rdfs:comment>Host of jdbc bridge.</rdfs:comment>
    <rdfs:domain rdf:resource="http://example.org/onto/class/yandex_mdb_clickhouse_cluster"/>
    <rdfs:range rdf:resource="http://www.w3.org/2001/XMLSchema#string"/>
  </owl:DatatypeProperty>
  <owl:DatatypeProperty rdf:about="http://example.org/onto/prop/yandex_mdb_clickhouse_cluster_port">
    <rdfs:label>port</rdfs:label>
    <rdfs:comment>Port of jdbc bridge. Default value: 9019.</rdfs:comment>
    <rdfs:domain rdf:resource="http://example.org/onto/class/yandex_mdb_clickhouse_cluster"/>
    <rdfs:range rdf:resource="http://www.w3.org/2001/XMLSchema#string"/>
  </owl:DatatypeProperty>
  <owl:DatatypeProperty rdf:about="http://example.org/onto/prop/yandex_mdb_clickhouse_cluster_auto_offset_reset">
    <rdfs:label>auto_offset_reset</rdfs:label>
    <rdfs:comment>Action to take when there is no initial offset in offset store or the desired offset is out of range: 'smallest','earliest' - automatically reset the offset to the smallest offset, 'largest','latest' - automatically reset the offset to the largest offset, 'error' - trigger an error (ERR__AUTO_OFFSET_RESET) which is retrieved by consuming messages and checking 'message->err'.</rdfs:comment>
    <rdfs:domain rdf:resource="http://example.org/onto/class/yandex_mdb_clickhouse_cluster"/>
    <rdfs:range rdf:resource="http://www.w3.org/2001/XMLSchema#string"/>
  </owl:DatatypeProperty>
  <owl:DatatypeProperty rdf:about="http://example.org/onto/prop/yandex_mdb_clickhouse_cluster_debug">
    <rdfs:label>debug</rdfs:label>
    <rdfs:comment>A comma-separated list of debug contexts to enable.</rdfs:comment>
    <rdfs:domain rdf:resource="http://example.org/onto/class/yandex_mdb_clickhouse_cluster"/>
    <rdfs:range rdf:resource="http://www.w3.org/2001/XMLSchema#string"/>
  </owl:DatatypeProperty>
  <owl:DatatypeProperty rdf:about="http://example.org/onto/prop/yandex_mdb_clickhouse_cluster_enable_ssl_certificate_verification">
    <rdfs:label>enable_ssl_certificate_verification</rdfs:label>
    <rdfs:comment>Enable verification of SSL certificates.</rdfs:comment>
    <rdfs:domain rdf:resource="http://example.org/onto/class/yandex_mdb_clickhouse_cluster"/>
    <rdfs:range rdf:resource="http://www.w3.org/2001/XMLSchema#string"/>
  </owl:DatatypeProperty>
  <owl:DatatypeProperty rdf:about="http://example.org/onto/prop/yandex_mdb_clickhouse_cluster_max_poll_interval_ms">
    <rdfs:label>max_poll_interval_ms</rdfs:label>
    <rdfs:comment>Maximum allowed time between calls to consume messages (e.g., `rd_kafka_consumer_poll()` for high-level consumers. If this interval is exceeded the consumer is considered failed and the group will rebalance in order to reassign the partitions to another consumer group member.</rdfs:comment>
    <rdfs:domain rdf:resource="http://example.org/onto/class/yandex_mdb_clickhouse_cluster"/>
    <rdfs:range rdf:resource="http://www.w3.org/2001/XMLSchema#string"/>
  </owl:DatatypeProperty>
  <owl:DatatypeProperty rdf:about="http://example.org/onto/prop/yandex_mdb_clickhouse_cluster_sasl_mechanism">
    <rdfs:label>sasl_mechanism</rdfs:label>
    <rdfs:comment>SASL mechanism used in kafka authentication.</rdfs:comment>
    <rdfs:domain rdf:resource="http://example.org/onto/class/yandex_mdb_clickhouse_cluster"/>
    <rdfs:range rdf:resource="http://www.w3.org/2001/XMLSchema#string"/>
  </owl:DatatypeProperty>
  <owl:DatatypeProperty rdf:about="http://example.org/onto/prop/yandex_mdb_clickhouse_cluster_sasl_password">
    <rdfs:label>sasl_password</rdfs:label>
    <rdfs:comment>User password on kafka server.</rdfs:comment>
    <rdfs:domain rdf:resource="http://example.org/onto/class/yandex_mdb_clickhouse_cluster"/>
    <rdfs:range rdf:resource="http://www.w3.org/2001/XMLSchema#string"/>
  </owl:DatatypeProperty>
  <owl:DatatypeProperty rdf:about="http://example.org/onto/prop/yandex_mdb_clickhouse_cluster_sasl_username">
    <rdfs:label>sasl_username</rdfs:label>
    <rdfs:comment>Username on kafka server.</rdfs:comment>
    <rdfs:domain rdf:resource="http://example.org/onto/class/yandex_mdb_clickhouse_cluster"/>
    <rdfs:range rdf:resource="http://www.w3.org/2001/XMLSchema#string"/>
  </owl:DatatypeProperty>
  <owl:DatatypeProperty rdf:about="http://example.org/onto/prop/yandex_mdb_clickhouse_cluster_security_protocol">
    <rdfs:label>security_protocol</rdfs:label>
    <rdfs:comment>Security protocol used to connect to kafka server.</rdfs:comment>
    <rdfs:domain rdf:resource="http://example.org/onto/class/yandex_mdb_clickhouse_cluster"/>
    <rdfs:range rdf:resource="http://www.w3.org/2001/XMLSchema#string"/>
  </owl:DatatypeProperty>
  <owl:DatatypeProperty rdf:about="http://example.org/onto/prop/yandex_mdb_clickhouse_cluster_session_timeout_ms">
    <rdfs:label>session_timeout_ms</rdfs:label>
    <rdfs:comment>Client group session and failure detection timeout. The consumer sends periodic heartbeats (heartbeat.interval.ms) to indicate its liveness to the broker. If no hearts are received by the broker for a group member within the session timeout, the broker will remove the consumer from the group and trigger a rebalance.</rdfs:comment>
    <rdfs:domain rdf:resource="http://example.org/onto/class/yandex_mdb_clickhouse_cluster"/>
    <rdfs:range rdf:resource="http://www.w3.org/2001/XMLSchema#string"/>
  </owl:DatatypeProperty>
  <owl:DatatypeProperty rdf:about="http://example.org/onto/prop/yandex_mdb_clickhouse_cluster_name">
    <rdfs:label>name</rdfs:label>
    <rdfs:comment>Kafka topic name.</rdfs:comment>
    <rdfs:domain rdf:resource="http://example.org/onto/class/yandex_mdb_clickhouse_cluster"/>
    <rdfs:range rdf:resource="http://www.w3.org/2001/XMLSchema#string"/>
  </owl:DatatypeProperty>
  <owl:DatatypeProperty rdf:about="http://example.org/onto/prop/yandex_mdb_clickhouse_cluster_auto_offset_reset">
    <rdfs:label>auto_offset_reset</rdfs:label>
    <rdfs:comment>Action to take when there is no initial offset in offset store or the desired offset is out of range: 'smallest','earliest' - automatically reset the offset to the smallest offset, 'largest','latest' - automatically reset the offset to the largest offset, 'error' - trigger an error (ERR__AUTO_OFFSET_RESET) which is retrieved by consuming messages and checking 'message->err'.</rdfs:comment>
    <rdfs:domain rdf:resource="http://example.org/onto/class/yandex_mdb_clickhouse_cluster"/>
    <rdfs:range rdf:resource="http://www.w3.org/2001/XMLSchema#string"/>
  </owl:DatatypeProperty>
  <owl:DatatypeProperty rdf:about="http://example.org/onto/prop/yandex_mdb_clickhouse_cluster_debug">
    <rdfs:label>debug</rdfs:label>
    <rdfs:comment>A comma-separated list of debug contexts to enable.</rdfs:comment>
    <rdfs:domain rdf:resource="http://example.org/onto/class/yandex_mdb_clickhouse_cluster"/>
    <rdfs:range rdf:resource="http://www.w3.org/2001/XMLSchema#string"/>
  </owl:DatatypeProperty>
  <owl:DatatypeProperty rdf:about="http://example.org/onto/prop/yandex_mdb_clickhouse_cluster_enable_ssl_certificate_verification">
    <rdfs:label>enable_ssl_certificate_verification</rdfs:label>
    <rdfs:comment>Enable verification of SSL certificates.</rdfs:comment>
    <rdfs:domain rdf:resource="http://example.org/onto/class/yandex_mdb_clickhouse_cluster"/>
    <rdfs:range rdf:resource="http://www.w3.org/2001/XMLSchema#string"/>
  </owl:DatatypeProperty>
  <owl:DatatypeProperty rdf:about="http://example.org/onto/prop/yandex_mdb_clickhouse_cluster_max_poll_interval_ms">
    <rdfs:label>max_poll_interval_ms</rdfs:label>
    <rdfs:comment>Maximum allowed time between calls to consume messages (e.g., `rd_kafka_consumer_poll()` for high-level consumers. If this interval is exceeded the consumer is considered failed and the group will rebalance in order to reassign the partitions to another consumer group member.</rdfs:comment>
    <rdfs:domain rdf:resource="http://example.org/onto/class/yandex_mdb_clickhouse_cluster"/>
    <rdfs:range rdf:resource="http://www.w3.org/2001/XMLSchema#string"/>
  </owl:DatatypeProperty>
  <owl:DatatypeProperty rdf:about="http://example.org/onto/prop/yandex_mdb_clickhouse_cluster_sasl_mechanism">
    <rdfs:label>sasl_mechanism</rdfs:label>
    <rdfs:comment>SASL mechanism used in kafka authentication.</rdfs:comment>
    <rdfs:domain rdf:resource="http://example.org/onto/class/yandex_mdb_clickhouse_cluster"/>
    <rdfs:range rdf:resource="http://www.w3.org/2001/XMLSchema#string"/>
  </owl:DatatypeProperty>
  <owl:DatatypeProperty rdf:about="http://example.org/onto/prop/yandex_mdb_clickhouse_cluster_sasl_password">
    <rdfs:label>sasl_password</rdfs:label>
    <rdfs:comment>User password on kafka server.</rdfs:comment>
    <rdfs:domain rdf:resource="http://example.org/onto/class/yandex_mdb_clickhouse_cluster"/>
    <rdfs:range rdf:resource="http://www.w3.org/2001/XMLSchema#string"/>
  </owl:DatatypeProperty>
  <owl:DatatypeProperty rdf:about="http://example.org/onto/prop/yandex_mdb_clickhouse_cluster_sasl_username">
    <rdfs:label>sasl_username</rdfs:label>
    <rdfs:comment>Username on kafka server.</rdfs:comment>
    <rdfs:domain rdf:resource="http://example.org/onto/class/yandex_mdb_clickhouse_cluster"/>
    <rdfs:range rdf:resource="http://www.w3.org/2001/XMLSchema#string"/>
  </owl:DatatypeProperty>
  <owl:DatatypeProperty rdf:about="http://example.org/onto/prop/yandex_mdb_clickhouse_cluster_security_protocol">
    <rdfs:label>security_protocol</rdfs:label>
    <rdfs:comment>Security protocol used to connect to kafka server.</rdfs:comment>
    <rdfs:domain rdf:resource="http://example.org/onto/class/yandex_mdb_clickhouse_cluster"/>
    <rdfs:range rdf:resource="http://www.w3.org/2001/XMLSchema#string"/>
  </owl:DatatypeProperty>
  <owl:DatatypeProperty rdf:about="http://example.org/onto/prop/yandex_mdb_clickhouse_cluster_session_timeout_ms">
    <rdfs:label>session_timeout_ms</rdfs:label>
    <rdfs:comment>Client group session and failure detection timeout. The consumer sends periodic heartbeats (heartbeat.interval.ms) to indicate its liveness to the broker. If no hearts are received by the broker for a group member within the session timeout, the broker will remove the consumer from the group and trigger a rebalance.</rdfs:comment>
    <rdfs:domain rdf:resource="http://example.org/onto/class/yandex_mdb_clickhouse_cluster"/>
    <rdfs:range rdf:resource="http://www.w3.org/2001/XMLSchema#string"/>
  </owl:DatatypeProperty>
  <owl:DatatypeProperty rdf:about="http://example.org/onto/prop/yandex_mdb_clickhouse_cluster_allow_remote_fs_zero_copy_replication">
    <rdfs:label>allow_remote_fs_zero_copy_replication</rdfs:label>
    <rdfs:comment>When this setting has a value greater than zero only a single replica starts the merge immediately if merged part on shared storage and allow_remote_fs_zero_copy_replication is enabled.</rdfs:comment>
    <rdfs:domain rdf:resource="http://example.org/onto/class/yandex_mdb_clickhouse_cluster"/>
    <rdfs:range rdf:resource="http://www.w3.org/2001/XMLSchema#string"/>
  </owl:DatatypeProperty>
  <owl:DatatypeProperty rdf:about="http://example.org/onto/prop/yandex_mdb_clickhouse_cluster_check_sample_column_is_correct">
    <rdfs:label>check_sample_column_is_correct</rdfs:label>
    <rdfs:comment>Enables the check at table creation, that the data type of a column for sampling or sampling expression is correct. The data type must be one of unsigned integer types: UInt8, UInt16, UInt32, UInt64. Default value: true.</rdfs:comment>
    <rdfs:domain rdf:resource="http://example.org/onto/class/yandex_mdb_clickhouse_cluster"/>
    <rdfs:range rdf:resource="http://www.w3.org/2001/XMLSchema#string"/>
  </owl:DatatypeProperty>
  <owl:DatatypeProperty rdf:about="http://example.org/onto/prop/yandex_mdb_clickhouse_cluster_cleanup_delay_period">
    <rdfs:label>cleanup_delay_period</rdfs:label>
    <rdfs:comment>Minimum period to clean old queue logs, blocks hashes and parts.</rdfs:comment>
    <rdfs:domain rdf:resource="http://example.org/onto/class/yandex_mdb_clickhouse_cluster"/>
    <rdfs:range rdf:resource="http://www.w3.org/2001/XMLSchema#string"/>
  </owl:DatatypeProperty>
  <owl:DatatypeProperty rdf:about="http://example.org/onto/prop/yandex_mdb_clickhouse_cluster_inactive_parts_to_delay_insert">
    <rdfs:label>inactive_parts_to_delay_insert</rdfs:label>
    <rdfs:comment>If the number of inactive parts in a single partition in the table at least that many the inactive_parts_to_delay_insert value, an INSERT artificially slows down. It is useful when a server fails to clean up parts quickly enough.</rdfs:comment>
    <rdfs:domain rdf:resource="http://example.org/onto/class/yandex_mdb_clickhouse_cluster"/>
    <rdfs:range rdf:resource="http://www.w3.org/2001/XMLSchema#string"/>
  </owl:DatatypeProperty>
  <owl:DatatypeProperty rdf:about="http://example.org/onto/prop/yandex_mdb_clickhouse_cluster_inactive_parts_to_throw_insert">
    <rdfs:label>inactive_parts_to_throw_insert</rdfs:label>
    <rdfs:comment>If the number of inactive parts in a single partition more than the inactive_parts_to_throw_insert value, INSERT is interrupted with the `Too many inactive parts (N). Parts cleaning are processing significantly slower than inserts` exception.</rdfs:comment>
    <rdfs:domain rdf:resource="http://example.org/onto/class/yandex_mdb_clickhouse_cluster"/>
    <rdfs:range rdf:resource="http://www.w3.org/2001/XMLSchema#string"/>
  </owl:DatatypeProperty>
  <owl:DatatypeProperty rdf:about="http://example.org/onto/prop/yandex_mdb_clickhouse_cluster_max_avg_part_size_for_too_many_parts">
    <rdfs:label>max_avg_part_size_for_too_many_parts</rdfs:label>
    <rdfs:comment>The `too many parts` check according to `parts_to_delay_insert` and `parts_to_throw_insert` will be active only if the average part size (in the relevant partition) is not larger than the specified threshold. If it is larger than the specified threshold, the INSERTs will be neither delayed or rejected. This allows to have hundreds of terabytes in a single table on a single server if the parts are successfully merged to larger parts. This does not affect the thresholds on inactive parts or total parts.</rdfs:comment>
    <rdfs:domain rdf:resource="http://example.org/onto/class/yandex_mdb_clickhouse_cluster"/>
    <rdfs:range rdf:resource="http://www.w3.org/2001/XMLSchema#string"/>
  </owl:DatatypeProperty>
  <owl:DatatypeProperty rdf:about="http://example.org/onto/prop/yandex_mdb_clickhouse_cluster_max_bytes_to_merge_at_max_space_in_pool">
    <rdfs:label>max_bytes_to_merge_at_max_space_in_pool</rdfs:label>
    <rdfs:comment>The maximum total parts size (in bytes) to be merged into one part, if there are enough resources available. max_bytes_to_merge_at_max_space_in_pool -- roughly corresponds to the maximum possible part size created by an automatic background merge.</rdfs:comment>
    <rdfs:domain rdf:resource="http://example.org/onto/class/yandex_mdb_clickhouse_cluster"/>
    <rdfs:range rdf:resource="http://www.w3.org/2001/XMLSchema#string"/>
  </owl:DatatypeProperty>
  <owl:DatatypeProperty rdf:about="http://example.org/onto/prop/yandex_mdb_clickhouse_cluster_max_bytes_to_merge_at_min_space_in_pool">
    <rdfs:label>max_bytes_to_merge_at_min_space_in_pool</rdfs:label>
    <rdfs:comment>Max bytes to merge at min space in pool: Maximum total size of a data part to merge when the number of free threads in the background pool is minimum.</rdfs:comment>
    <rdfs:domain rdf:resource="http://example.org/onto/class/yandex_mdb_clickhouse_cluster"/>
    <rdfs:range rdf:resource="http://www.w3.org/2001/XMLSchema#string"/>
  </owl:DatatypeProperty>
  <owl:DatatypeProperty rdf:about="http://example.org/onto/prop/yandex_mdb_clickhouse_cluster_max_cleanup_delay_period">
    <rdfs:label>max_cleanup_delay_period</rdfs:label>
    <rdfs:comment>Maximum period to clean old queue logs, blocks hashes and parts. Default value: 300 seconds.</rdfs:comment>
    <rdfs:domain rdf:resource="http://example.org/onto/class/yandex_mdb_clickhouse_cluster"/>
    <rdfs:range rdf:resource="http://www.w3.org/2001/XMLSchema#string"/>
  </owl:DatatypeProperty>
  <owl:DatatypeProperty rdf:about="http://example.org/onto/prop/yandex_mdb_clickhouse_cluster_max_merge_selecting_sleep_ms">
    <rdfs:label>max_merge_selecting_sleep_ms</rdfs:label>
    <rdfs:comment>Maximum sleep time for merge selecting, a lower setting will trigger selecting tasks in background_schedule_pool frequently which result in large amount of requests to zookeeper in large-scale clusters. Default value: 60000 milliseconds (60 seconds).</rdfs:comment>
    <rdfs:domain rdf:resource="http://example.org/onto/class/yandex_mdb_clickhouse_cluster"/>
    <rdfs:range rdf:resource="http://www.w3.org/2001/XMLSchema#string"/>
  </owl:DatatypeProperty>
  <owl:DatatypeProperty rdf:about="http://example.org/onto/prop/yandex_mdb_clickhouse_cluster_max_number_of_merges_with_ttl_in_pool">
    <rdfs:label>max_number_of_merges_with_ttl_in_pool</rdfs:label>
    <rdfs:comment>When there is more than specified number of merges with TTL entries in pool, do not assign new merge with TTL.</rdfs:comment>
    <rdfs:domain rdf:resource="http://example.org/onto/class/yandex_mdb_clickhouse_cluster"/>
    <rdfs:range rdf:resource="http://www.w3.org/2001/XMLSchema#string"/>
  </owl:DatatypeProperty>
  <owl:DatatypeProperty rdf:about="http://example.org/onto/prop/yandex_mdb_clickhouse_cluster_max_parts_in_total">
    <rdfs:label>max_parts_in_total</rdfs:label>
    <rdfs:comment>Maximum number of parts in all partitions.</rdfs:comment>
    <rdfs:domain rdf:resource="http://example.org/onto/class/yandex_mdb_clickhouse_cluster"/>
    <rdfs:range rdf:resource="http://www.w3.org/2001/XMLSchema#string"/>
  </owl:DatatypeProperty>
  <owl:DatatypeProperty rdf:about="http://example.org/onto/prop/yandex_mdb_clickhouse_cluster_max_replicated_merges_in_queue">
    <rdfs:label>max_replicated_merges_in_queue</rdfs:label>
    <rdfs:comment>Max replicated merges in queue: Maximum number of merge tasks that can be in the ReplicatedMergeTree queue at the same time.</rdfs:comment>
    <rdfs:domain rdf:resource="http://example.org/onto/class/yandex_mdb_clickhouse_cluster"/>
    <rdfs:range rdf:resource="http://www.w3.org/2001/XMLSchema#string"/>
  </owl:DatatypeProperty>
  <owl:DatatypeProperty rdf:about="http://example.org/onto/prop/yandex_mdb_clickhouse_cluster_merge_max_block_size">
    <rdfs:label>merge_max_block_size</rdfs:label>
    <rdfs:comment>The number of rows that are read from the merged parts into memory. Default value: 8192.</rdfs:comment>
    <rdfs:domain rdf:resource="http://example.org/onto/class/yandex_mdb_clickhouse_cluster"/>
    <rdfs:range rdf:resource="http://www.w3.org/2001/XMLSchema#string"/>
  </owl:DatatypeProperty>
  <owl:DatatypeProperty rdf:about="http://example.org/onto/prop/yandex_mdb_clickhouse_cluster_merge_selecting_sleep_ms">
    <rdfs:label>merge_selecting_sleep_ms</rdfs:label>
    <rdfs:comment>Sleep time for merge selecting when no part is selected. A lower setting triggers selecting tasks in background_schedule_pool frequently, which results in a large number of requests to ClickHouse Keeper in large-scale clusters.</rdfs:comment>
    <rdfs:domain rdf:resource="http://example.org/onto/class/yandex_mdb_clickhouse_cluster"/>
    <rdfs:range rdf:resource="http://www.w3.org/2001/XMLSchema#string"/>
  </owl:DatatypeProperty>
  <owl:DatatypeProperty rdf:about="http://example.org/onto/prop/yandex_mdb_clickhouse_cluster_merge_with_recompression_ttl_timeout">
    <rdfs:label>merge_with_recompression_ttl_timeout</rdfs:label>
    <rdfs:comment>Minimum delay in seconds before repeating a merge with recompression TTL. Default value: 14400 seconds (4 hours).</rdfs:comment>
    <rdfs:domain rdf:resource="http://example.org/onto/class/yandex_mdb_clickhouse_cluster"/>
    <rdfs:range rdf:resource="http://www.w3.org/2001/XMLSchema#string"/>
  </owl:DatatypeProperty>
  <owl:DatatypeProperty rdf:about="http://example.org/onto/prop/yandex_mdb_clickhouse_cluster_merge_with_ttl_timeout">
    <rdfs:label>merge_with_ttl_timeout</rdfs:label>
    <rdfs:comment>Minimum delay in seconds before repeating a merge with delete TTL. Default value: 14400 seconds (4 hours).</rdfs:comment>
    <rdfs:domain rdf:resource="http://example.org/onto/class/yandex_mdb_clickhouse_cluster"/>
    <rdfs:range rdf:resource="http://www.w3.org/2001/XMLSchema#string"/>
  </owl:DatatypeProperty>
  <owl:DatatypeProperty rdf:about="http://example.org/onto/prop/yandex_mdb_clickhouse_cluster_min_age_to_force_merge_on_partition_only">
    <rdfs:label>min_age_to_force_merge_on_partition_only</rdfs:label>
    <rdfs:comment>Whether min_age_to_force_merge_seconds should be applied only on the entire partition and not on subset.</rdfs:comment>
    <rdfs:domain rdf:resource="http://example.org/onto/class/yandex_mdb_clickhouse_cluster"/>
    <rdfs:range rdf:resource="http://www.w3.org/2001/XMLSchema#string"/>
  </owl:DatatypeProperty>
  <owl:DatatypeProperty rdf:about="http://example.org/onto/prop/yandex_mdb_clickhouse_cluster_min_age_to_force_merge_seconds">
    <rdfs:label>min_age_to_force_merge_seconds</rdfs:label>
    <rdfs:comment>Merge parts if every part in the range is older than the value of `min_age_to_force_merge_seconds`.</rdfs:comment>
    <rdfs:domain rdf:resource="http://example.org/onto/class/yandex_mdb_clickhouse_cluster"/>
    <rdfs:range rdf:resource="http://www.w3.org/2001/XMLSchema#string"/>
  </owl:DatatypeProperty>
  <owl:DatatypeProperty rdf:about="http://example.org/onto/prop/yandex_mdb_clickhouse_cluster_min_bytes_for_wide_part">
    <rdfs:label>min_bytes_for_wide_part</rdfs:label>
    <rdfs:comment>Minimum number of bytes in a data part that can be stored in Wide format. You can set one, both or none of these settings.</rdfs:comment>
    <rdfs:domain rdf:resource="http://example.org/onto/class/yandex_mdb_clickhouse_cluster"/>
    <rdfs:range rdf:resource="http://www.w3.org/2001/XMLSchema#string"/>
  </owl:DatatypeProperty>
  <owl:DatatypeProperty rdf:about="http://example.org/onto/prop/yandex_mdb_clickhouse_cluster_min_rows_for_wide_part">
    <rdfs:label>min_rows_for_wide_part</rdfs:label>
    <rdfs:comment>Minimum number of rows in a data part that can be stored in Wide format. You can set one, both or none of these settings.</rdfs:comment>
    <rdfs:domain rdf:resource="http://example.org/onto/class/yandex_mdb_clickhouse_cluster"/>
    <rdfs:range rdf:resource="http://www.w3.org/2001/XMLSchema#string"/>
  </owl:DatatypeProperty>
  <owl:DatatypeProperty rdf:about="http://example.org/onto/prop/yandex_mdb_clickhouse_cluster_number_of_free_entries_in_pool_to_execute_mutation">
    <rdfs:label>number_of_free_entries_in_pool_to_execute_mutation</rdfs:label>
    <rdfs:comment>When there is less than specified number of free entries in pool, do not execute part mutations. This is to leave free threads for regular merges and avoid `Too many parts`. Default value: 20.</rdfs:comment>
    <rdfs:domain rdf:resource="http://example.org/onto/class/yandex_mdb_clickhouse_cluster"/>
    <rdfs:range rdf:resource="http://www.w3.org/2001/XMLSchema#string"/>
  </owl:DatatypeProperty>
  <owl:DatatypeProperty rdf:about="http://example.org/onto/prop/yandex_mdb_clickhouse_cluster_number_of_free_entries_in_pool_to_lower_max_size_of_merge">
    <rdfs:label>number_of_free_entries_in_pool_to_lower_max_size_of_merge</rdfs:label>
    <rdfs:comment>Number of free entries in pool to lower max size of merge: Threshold value of free entries in the pool. If the number of entries in the pool falls below this value, ClickHouse reduces the maximum size of a data part to merge. This helps handle small merges faster, rather than filling the pool with lengthy merges.</rdfs:comment>
    <rdfs:domain rdf:resource="http://example.org/onto/class/yandex_mdb_clickhouse_cluster"/>
    <rdfs:range rdf:resource="http://www.w3.org/2001/XMLSchema#string"/>
  </owl:DatatypeProperty>
  <owl:DatatypeProperty rdf:about="http://example.org/onto/prop/yandex_mdb_clickhouse_cluster_parts_to_delay_insert">
    <rdfs:label>parts_to_delay_insert</rdfs:label>
    <rdfs:comment>Parts to delay insert: Number of active data parts in a table, on exceeding which ClickHouse starts artificially reduce the rate of inserting data into the table</rdfs:comment>
    <rdfs:domain rdf:resource="http://example.org/onto/class/yandex_mdb_clickhouse_cluster"/>
    <rdfs:range rdf:resource="http://www.w3.org/2001/XMLSchema#string"/>
  </owl:DatatypeProperty>
  <owl:DatatypeProperty rdf:about="http://example.org/onto/prop/yandex_mdb_clickhouse_cluster_parts_to_throw_insert">
    <rdfs:label>parts_to_throw_insert</rdfs:label>
    <rdfs:comment>Parts to throw insert: Threshold value of active data parts in a table, on exceeding which ClickHouse throws the 'Too many parts ...' exception.</rdfs:comment>
    <rdfs:domain rdf:resource="http://example.org/onto/class/yandex_mdb_clickhouse_cluster"/>
    <rdfs:range rdf:resource="http://www.w3.org/2001/XMLSchema#string"/>
  </owl:DatatypeProperty>
  <owl:DatatypeProperty rdf:about="http://example.org/onto/prop/yandex_mdb_clickhouse_cluster_replicated_deduplication_window">
    <rdfs:label>replicated_deduplication_window</rdfs:label>
    <rdfs:comment>Replicated deduplication window: Number of recent hash blocks that ZooKeeper will store (the old ones will be deleted).</rdfs:comment>
    <rdfs:domain rdf:resource="http://example.org/onto/class/yandex_mdb_clickhouse_cluster"/>
    <rdfs:range rdf:resource="http://www.w3.org/2001/XMLSchema#string"/>
  </owl:DatatypeProperty>
  <owl:DatatypeProperty rdf:about="http://example.org/onto/prop/yandex_mdb_clickhouse_cluster_replicated_deduplication_window_seconds">
    <rdfs:label>replicated_deduplication_window_seconds</rdfs:label>
    <rdfs:comment>Replicated deduplication window seconds: Time during which ZooKeeper stores the hash blocks (the old ones wil be deleted).</rdfs:comment>
    <rdfs:domain rdf:resource="http://example.org/onto/class/yandex_mdb_clickhouse_cluster"/>
    <rdfs:range rdf:resource="http://www.w3.org/2001/XMLSchema#string"/>
  </owl:DatatypeProperty>
  <owl:DatatypeProperty rdf:about="http://example.org/onto/prop/yandex_mdb_clickhouse_cluster_ttl_only_drop_parts">
    <rdfs:label>ttl_only_drop_parts</rdfs:label>
    <rdfs:comment>Enables zero-copy replication when a replica is located on a remote filesystem.</rdfs:comment>
    <rdfs:domain rdf:resource="http://example.org/onto/class/yandex_mdb_clickhouse_cluster"/>
    <rdfs:range rdf:resource="http://www.w3.org/2001/XMLSchema#string"/>
  </owl:DatatypeProperty>
  <owl:DatatypeProperty rdf:about="http://example.org/onto/prop/yandex_mdb_clickhouse_cluster_max_entries">
    <rdfs:label>max_entries</rdfs:label>
    <rdfs:comment>The maximum number of SELECT query results stored in the cache. Default value: 1024.</rdfs:comment>
    <rdfs:domain rdf:resource="http://example.org/onto/class/yandex_mdb_clickhouse_cluster"/>
    <rdfs:range rdf:resource="http://www.w3.org/2001/XMLSchema#string"/>
  </owl:DatatypeProperty>
  <owl:DatatypeProperty rdf:about="http://example.org/onto/prop/yandex_mdb_clickhouse_cluster_max_entry_size_in_bytes">
    <rdfs:label>max_entry_size_in_bytes</rdfs:label>
    <rdfs:comment>The maximum size in bytes SELECT query results may have to be saved in the cache. Default value: 1048576 (1 MiB).</rdfs:comment>
    <rdfs:domain rdf:resource="http://example.org/onto/class/yandex_mdb_clickhouse_cluster"/>
    <rdfs:range rdf:resource="http://www.w3.org/2001/XMLSchema#string"/>
  </owl:DatatypeProperty>
  <owl:DatatypeProperty rdf:about="http://example.org/onto/prop/yandex_mdb_clickhouse_cluster_max_entry_size_in_rows">
    <rdfs:label>max_entry_size_in_rows</rdfs:label>
    <rdfs:comment>The maximum number of rows SELECT query results may have to be saved in the cache. Default value: 30000000 (30 mil).</rdfs:comment>
    <rdfs:domain rdf:resource="http://example.org/onto/class/yandex_mdb_clickhouse_cluster"/>
    <rdfs:range rdf:resource="http://www.w3.org/2001/XMLSchema#string"/>
  </owl:DatatypeProperty>
  <owl:DatatypeProperty rdf:about="http://example.org/onto/prop/yandex_mdb_clickhouse_cluster_max_size_in_bytes">
    <rdfs:label>max_size_in_bytes</rdfs:label>
    <rdfs:comment>The maximum cache size in bytes. 0 means the query cache is disabled. Default value: 1073741824 (1 GiB).</rdfs:comment>
    <rdfs:domain rdf:resource="http://example.org/onto/class/yandex_mdb_clickhouse_cluster"/>
    <rdfs:range rdf:resource="http://www.w3.org/2001/XMLSchema#string"/>
  </owl:DatatypeProperty>
  <owl:DatatypeProperty rdf:about="http://example.org/onto/prop/yandex_mdb_clickhouse_cluster_name">
    <rdfs:label>name</rdfs:label>
    <rdfs:comment>Name for the rule.</rdfs:comment>
    <rdfs:domain rdf:resource="http://example.org/onto/class/yandex_mdb_clickhouse_cluster"/>
    <rdfs:range rdf:resource="http://www.w3.org/2001/XMLSchema#string"/>
  </owl:DatatypeProperty>
  <owl:DatatypeProperty rdf:about="http://example.org/onto/prop/yandex_mdb_clickhouse_cluster_regexp">
    <rdfs:label>regexp</rdfs:label>
    <rdfs:comment>RE2 compatible regular expression.</rdfs:comment>
    <rdfs:domain rdf:resource="http://example.org/onto/class/yandex_mdb_clickhouse_cluster"/>
    <rdfs:range rdf:resource="http://www.w3.org/2001/XMLSchema#string"/>
  </owl:DatatypeProperty>
  <owl:DatatypeProperty rdf:about="http://example.org/onto/prop/yandex_mdb_clickhouse_cluster_replace">
    <rdfs:label>replace</rdfs:label>
    <rdfs:comment>Substitution string for sensitive data. Default value: six asterisks.</rdfs:comment>
    <rdfs:domain rdf:resource="http://example.org/onto/class/yandex_mdb_clickhouse_cluster"/>
    <rdfs:range rdf:resource="http://www.w3.org/2001/XMLSchema#string"/>
  </owl:DatatypeProperty>
  <owl:DatatypeProperty rdf:about="http://example.org/onto/prop/yandex_mdb_clickhouse_cluster_password">
    <rdfs:label>password</rdfs:label>
    <rdfs:comment>RabbitMQ user password.</rdfs:comment>
    <rdfs:domain rdf:resource="http://example.org/onto/class/yandex_mdb_clickhouse_cluster"/>
    <rdfs:range rdf:resource="http://www.w3.org/2001/XMLSchema#string"/>
  </owl:DatatypeProperty>
  <owl:DatatypeProperty rdf:about="http://example.org/onto/prop/yandex_mdb_clickhouse_cluster_username">
    <rdfs:label>username</rdfs:label>
    <rdfs:comment>RabbitMQ username.</rdfs:comment>
    <rdfs:domain rdf:resource="http://example.org/onto/class/yandex_mdb_clickhouse_cluster"/>
    <rdfs:range rdf:resource="http://www.w3.org/2001/XMLSchema#string"/>
  </owl:DatatypeProperty>
  <owl:DatatypeProperty rdf:about="http://example.org/onto/prop/yandex_mdb_clickhouse_cluster_vhost">
    <rdfs:label>vhost</rdfs:label>
    <rdfs:comment>RabbitMQ vhost. Default: `\`.</rdfs:comment>
    <rdfs:domain rdf:resource="http://example.org/onto/class/yandex_mdb_clickhouse_cluster"/>
    <rdfs:range rdf:resource="http://www.w3.org/2001/XMLSchema#string"/>
  </owl:DatatypeProperty>
  <owl:DatatypeProperty rdf:about="http://example.org/onto/prop/yandex_mdb_clickhouse_cluster_disk_size">
    <rdfs:label>disk_size</rdfs:label>
    <rdfs:comment>Volume of the storage available to a ClickHouse host, in gigabytes.</rdfs:comment>
    <rdfs:domain rdf:resource="http://example.org/onto/class/yandex_mdb_clickhouse_cluster"/>
    <rdfs:range rdf:resource="http://www.w3.org/2001/XMLSchema#string"/>
  </owl:DatatypeProperty>
  <owl:DatatypeProperty rdf:about="http://example.org/onto/prop/yandex_mdb_clickhouse_cluster_disk_type_id">
    <rdfs:label>disk_type_id</rdfs:label>
    <rdfs:comment>Type of the storage of ClickHouse hosts. For more information see [the official documentation](https://yandex.cloud/docs/managed-clickhouse/concepts/storage).</rdfs:comment>
    <rdfs:domain rdf:resource="http://example.org/onto/class/yandex_mdb_clickhouse_cluster"/>
    <rdfs:range rdf:resource="http://www.w3.org/2001/XMLSchema#string"/>
  </owl:DatatypeProperty>
  <owl:DatatypeProperty rdf:about="http://example.org/onto/prop/yandex_mdb_clickhouse_cluster_resource_preset_id">
    <rdfs:label>resource_preset_id</rdfs:label>
    <rdfs:comment>The ID of the preset for computational resources available to a ClickHouse host (CPU, memory etc.). For more information, see [the official documentation](https://yandex.cloud/docs/managed-clickhouse/concepts).</rdfs:comment>
    <rdfs:domain rdf:resource="http://example.org/onto/class/yandex_mdb_clickhouse_cluster"/>
    <rdfs:range rdf:resource="http://www.w3.org/2001/XMLSchema#string"/>
  </owl:DatatypeProperty>
  <owl:DatatypeProperty rdf:about="http://example.org/onto/prop/yandex_mdb_clickhouse_cluster_data_cache_enabled">
    <rdfs:label>data_cache_enabled</rdfs:label>
    <rdfs:comment>Enables temporary storage in the cluster repository of data requested from the object repository.</rdfs:comment>
    <rdfs:domain rdf:resource="http://example.org/onto/class/yandex_mdb_clickhouse_cluster"/>
    <rdfs:range rdf:resource="http://www.w3.org/2001/XMLSchema#string"/>
  </owl:DatatypeProperty>
  <owl:DatatypeProperty rdf:about="http://example.org/onto/prop/yandex_mdb_clickhouse_cluster_data_cache_max_size">
    <rdfs:label>data_cache_max_size</rdfs:label>
    <rdfs:comment>Defines the maximum amount of memory (in bytes) allocated in the cluster storage for temporary storage of data requested from the object storage.</rdfs:comment>
    <rdfs:domain rdf:resource="http://example.org/onto/class/yandex_mdb_clickhouse_cluster"/>
    <rdfs:range rdf:resource="http://www.w3.org/2001/XMLSchema#string"/>
  </owl:DatatypeProperty>
  <owl:DatatypeProperty rdf:about="http://example.org/onto/prop/yandex_mdb_clickhouse_cluster_enabled">
    <rdfs:label>enabled</rdfs:label>
    <rdfs:comment>Whether to use Yandex Object Storage for storing ClickHouse data. Can be either `true` or `false`.</rdfs:comment>
    <rdfs:domain rdf:resource="http://example.org/onto/class/yandex_mdb_clickhouse_cluster"/>
    <rdfs:range rdf:resource="http://www.w3.org/2001/XMLSchema#string"/>
  </owl:DatatypeProperty>
  <owl:DatatypeProperty rdf:about="http://example.org/onto/prop/yandex_mdb_clickhouse_cluster_move_factor">
    <rdfs:label>move_factor</rdfs:label>
    <rdfs:comment>Sets the minimum free space ratio in the cluster storage. If the free space is lower than this value, the data is transferred to Yandex Object Storage. Acceptable values are 0 to 1, inclusive.</rdfs:comment>
    <rdfs:domain rdf:resource="http://example.org/onto/class/yandex_mdb_clickhouse_cluster"/>
    <rdfs:range rdf:resource="http://www.w3.org/2001/XMLSchema#string"/>
  </owl:DatatypeProperty>
  <owl:DatatypeProperty rdf:about="http://example.org/onto/prop/yandex_mdb_clickhouse_cluster_prefer_not_to_merge">
    <rdfs:label>prefer_not_to_merge</rdfs:label>
    <rdfs:comment>Disables merging of data parts in `Yandex Object Storage`.</rdfs:comment>
    <rdfs:domain rdf:resource="http://example.org/onto/class/yandex_mdb_clickhouse_cluster"/>
    <rdfs:range rdf:resource="http://www.w3.org/2001/XMLSchema#string"/>
  </owl:DatatypeProperty>
  <owl:DatatypeProperty rdf:about="http://example.org/onto/prop/yandex_mdb_clickhouse_cluster_name">
    <rdfs:label>name</rdfs:label>
    <rdfs:comment>The name of the database.</rdfs:comment>
    <rdfs:domain rdf:resource="http://example.org/onto/class/yandex_mdb_clickhouse_cluster"/>
    <rdfs:range rdf:resource="http://www.w3.org/2001/XMLSchema#string"/>
  </owl:DatatypeProperty>
  <owl:DatatypeProperty rdf:about="http://example.org/onto/prop/yandex_mdb_clickhouse_cluster_name">
    <rdfs:label>name</rdfs:label>
    <rdfs:comment>The name of the format schema.</rdfs:comment>
    <rdfs:domain rdf:resource="http://example.org/onto/class/yandex_mdb_clickhouse_cluster"/>
    <rdfs:range rdf:resource="http://www.w3.org/2001/XMLSchema#string"/>
  </owl:DatatypeProperty>
  <owl:DatatypeProperty rdf:about="http://example.org/onto/prop/yandex_mdb_clickhouse_cluster_type">
    <rdfs:label>type</rdfs:label>
    <rdfs:comment>Type of the format schema.</rdfs:comment>
    <rdfs:domain rdf:resource="http://example.org/onto/class/yandex_mdb_clickhouse_cluster"/>
    <rdfs:range rdf:resource="http://www.w3.org/2001/XMLSchema#string"/>
  </owl:DatatypeProperty>
  <owl:DatatypeProperty rdf:about="http://example.org/onto/prop/yandex_mdb_clickhouse_cluster_uri">
    <rdfs:label>uri</rdfs:label>
    <rdfs:comment>Format schema file URL. You can only use format schemas stored in Yandex Object Storage.</rdfs:comment>
    <rdfs:domain rdf:resource="http://example.org/onto/class/yandex_mdb_clickhouse_cluster"/>
    <rdfs:range rdf:resource="http://www.w3.org/2001/XMLSchema#string"/>
  </owl:DatatypeProperty>
  <owl:DatatypeProperty rdf:about="http://example.org/onto/prop/yandex_mdb_clickhouse_cluster_assign_public_ip">
    <rdfs:label>assign_public_ip</rdfs:label>
    <rdfs:comment>Sets whether the host should get a public IP address on creation. Can be either `true` or `false`.</rdfs:comment>
    <rdfs:domain rdf:resource="http://example.org/onto/class/yandex_mdb_clickhouse_cluster"/>
    <rdfs:range rdf:resource="http://www.w3.org/2001/XMLSchema#string"/>
  </owl:DatatypeProperty>
  <owl:DatatypeProperty rdf:about="http://example.org/onto/prop/yandex_mdb_clickhouse_cluster_fqdn">
    <rdfs:label>fqdn</rdfs:label>
    <rdfs:comment>The fully qualified domain name of the host.</rdfs:comment>
    <rdfs:domain rdf:resource="http://example.org/onto/class/yandex_mdb_clickhouse_cluster"/>
    <rdfs:range rdf:resource="http://www.w3.org/2001/XMLSchema#string"/>
  </owl:DatatypeProperty>
  <owl:DatatypeProperty rdf:about="http://example.org/onto/prop/yandex_mdb_clickhouse_cluster_shard_name">
    <rdfs:label>shard_name</rdfs:label>
    <rdfs:comment>The name of the shard to which the host belongs.</rdfs:comment>
    <rdfs:domain rdf:resource="http://example.org/onto/class/yandex_mdb_clickhouse_cluster"/>
    <rdfs:range rdf:resource="http://www.w3.org/2001/XMLSchema#string"/>
  </owl:DatatypeProperty>
  <owl:DatatypeProperty rdf:about="http://example.org/onto/prop/yandex_mdb_clickhouse_cluster_subnet_id">
    <rdfs:label>subnet_id</rdfs:label>
    <rdfs:comment>The ID of the subnet, to which the host belongs. The subnet must be a part of the network to which the cluster belongs.</rdfs:comment>
    <rdfs:domain rdf:resource="http://example.org/onto/class/yandex_mdb_clickhouse_cluster"/>
    <rdfs:range rdf:resource="http://www.w3.org/2001/XMLSchema#string"/>
  </owl:DatatypeProperty>
  <owl:DatatypeProperty rdf:about="http://example.org/onto/prop/yandex_mdb_clickhouse_cluster_type">
    <rdfs:label>type</rdfs:label>
    <rdfs:comment>The type of the host to be deployed. Can be either `CLICKHOUSE` or `ZOOKEEPER`.</rdfs:comment>
    <rdfs:domain rdf:resource="http://example.org/onto/class/yandex_mdb_clickhouse_cluster"/>
    <rdfs:range rdf:resource="http://www.w3.org/2001/XMLSchema#string"/>
  </owl:DatatypeProperty>
  <owl:DatatypeProperty rdf:about="http://example.org/onto/prop/yandex_mdb_clickhouse_cluster_zone">
    <rdfs:label>zone</rdfs:label>
    <rdfs:comment>The [availability zone](https://yandex.cloud/docs/overview/concepts/geo-scope) where resource is located. If it is not provided, the default provider zone will be used.</rdfs:comment>
    <rdfs:domain rdf:resource="http://example.org/onto/class/yandex_mdb_clickhouse_cluster"/>
    <rdfs:range rdf:resource="http://www.w3.org/2001/XMLSchema#string"/>
  </owl:DatatypeProperty>
  <owl:DatatypeProperty rdf:about="http://example.org/onto/prop/yandex_mdb_clickhouse_cluster_day">
    <rdfs:label>day</rdfs:label>
    <rdfs:comment>Day of week for maintenance window if window type is weekly. Possible values: `MON`, `TUE`, `WED`, `THU`, `FRI`, `SAT`, `SUN`.</rdfs:comment>
    <rdfs:domain rdf:resource="http://example.org/onto/class/yandex_mdb_clickhouse_cluster"/>
    <rdfs:range rdf:resource="http://www.w3.org/2001/XMLSchema#string"/>
  </owl:DatatypeProperty>
  <owl:DatatypeProperty rdf:about="http://example.org/onto/prop/yandex_mdb_clickhouse_cluster_hour">
    <rdfs:label>hour</rdfs:label>
    <rdfs:comment>Hour of day in UTC time zone (1-24) for maintenance window if window type is weekly.</rdfs:comment>
    <rdfs:domain rdf:resource="http://example.org/onto/class/yandex_mdb_clickhouse_cluster"/>
    <rdfs:range rdf:resource="http://www.w3.org/2001/XMLSchema#string"/>
  </owl:DatatypeProperty>
  <owl:DatatypeProperty rdf:about="http://example.org/onto/prop/yandex_mdb_clickhouse_cluster_type">
    <rdfs:label>type</rdfs:label>
    <rdfs:comment>Type of maintenance window. Can be either `ANYTIME` or `WEEKLY`. A day and hour of window need to be specified with weekly window.</rdfs:comment>
    <rdfs:domain rdf:resource="http://example.org/onto/class/yandex_mdb_clickhouse_cluster"/>
    <rdfs:range rdf:resource="http://www.w3.org/2001/XMLSchema#string"/>
  </owl:DatatypeProperty>
  <owl:DatatypeProperty rdf:about="http://example.org/onto/prop/yandex_mdb_clickhouse_cluster_name">
    <rdfs:label>name</rdfs:label>
    <rdfs:comment>The name of the ml model.</rdfs:comment>
    <rdfs:domain rdf:resource="http://example.org/onto/class/yandex_mdb_clickhouse_cluster"/>
    <rdfs:range rdf:resource="http://www.w3.org/2001/XMLSchema#string"/>
  </owl:DatatypeProperty>
  <owl:DatatypeProperty rdf:about="http://example.org/onto/prop/yandex_mdb_clickhouse_cluster_type">
    <rdfs:label>type</rdfs:label>
    <rdfs:comment>Type of the model.</rdfs:comment>
    <rdfs:domain rdf:resource="http://example.org/onto/class/yandex_mdb_clickhouse_cluster"/>
    <rdfs:range rdf:resource="http://www.w3.org/2001/XMLSchema#string"/>
  </owl:DatatypeProperty>
  <owl:DatatypeProperty rdf:about="http://example.org/onto/prop/yandex_mdb_clickhouse_cluster_uri">
    <rdfs:label>uri</rdfs:label>
    <rdfs:comment>Model file URL. You can only use models stored in Yandex Object Storage.</rdfs:comment>
    <rdfs:domain rdf:resource="http://example.org/onto/class/yandex_mdb_clickhouse_cluster"/>
    <rdfs:range rdf:resource="http://www.w3.org/2001/XMLSchema#string"/>
  </owl:DatatypeProperty>
  <owl:DatatypeProperty rdf:about="http://example.org/onto/prop/yandex_mdb_clickhouse_cluster_name">
    <rdfs:label>name</rdfs:label>
    <rdfs:comment>The name of shard.</rdfs:comment>
    <rdfs:domain rdf:resource="http://example.org/onto/class/yandex_mdb_clickhouse_cluster"/>
    <rdfs:range rdf:resource="http://www.w3.org/2001/XMLSchema#string"/>
  </owl:DatatypeProperty>
  <owl:DatatypeProperty rdf:about="http://example.org/onto/prop/yandex_mdb_clickhouse_cluster_weight">
    <rdfs:label>weight</rdfs:label>
    <rdfs:comment>The weight of shard.</rdfs:comment>
    <rdfs:domain rdf:resource="http://example.org/onto/class/yandex_mdb_clickhouse_cluster"/>
    <rdfs:range rdf:resource="http://www.w3.org/2001/XMLSchema#string"/>
  </owl:DatatypeProperty>
  <owl:DatatypeProperty rdf:about="http://example.org/onto/prop/yandex_mdb_clickhouse_cluster_disk_size">
    <rdfs:label>disk_size</rdfs:label>
    <rdfs:comment>Volume of the storage available to a ClickHouse host, in gigabytes.</rdfs:comment>
    <rdfs:domain rdf:resource="http://example.org/onto/class/yandex_mdb_clickhouse_cluster"/>
    <rdfs:range rdf:resource="http://www.w3.org/2001/XMLSchema#string"/>
  </owl:DatatypeProperty>
  <owl:DatatypeProperty rdf:about="http://example.org/onto/prop/yandex_mdb_clickhouse_cluster_disk_type_id">
    <rdfs:label>disk_type_id</rdfs:label>
    <rdfs:comment>Type of the storage of ClickHouse hosts. For more information see [the official documentation](https://yandex.cloud/docs/managed-clickhouse/concepts/storage).</rdfs:comment>
    <rdfs:domain rdf:resource="http://example.org/onto/class/yandex_mdb_clickhouse_cluster"/>
    <rdfs:range rdf:resource="http://www.w3.org/2001/XMLSchema#string"/>
  </owl:DatatypeProperty>
  <owl:DatatypeProperty rdf:about="http://example.org/onto/prop/yandex_mdb_clickhouse_cluster_resource_preset_id">
    <rdfs:label>resource_preset_id</rdfs:label>
    <rdfs:comment>The ID of the preset for computational resources available to a ClickHouse host (CPU, memory etc.). For more information, see [the official documentation](https://yandex.cloud/docs/managed-clickhouse/concepts).</rdfs:comment>
    <rdfs:domain rdf:resource="http://example.org/onto/class/yandex_mdb_clickhouse_cluster"/>
    <rdfs:range rdf:resource="http://www.w3.org/2001/XMLSchema#string"/>
  </owl:DatatypeProperty>
  <owl:DatatypeProperty rdf:about="http://example.org/onto/prop/yandex_mdb_clickhouse_cluster_description">
    <rdfs:label>description</rdfs:label>
    <rdfs:comment>Description of the shard group.</rdfs:comment>
    <rdfs:domain rdf:resource="http://example.org/onto/class/yandex_mdb_clickhouse_cluster"/>
    <rdfs:range rdf:resource="http://www.w3.org/2001/XMLSchema#string"/>
  </owl:DatatypeProperty>
  <owl:DatatypeProperty rdf:about="http://example.org/onto/prop/yandex_mdb_clickhouse_cluster_name">
    <rdfs:label>name</rdfs:label>
    <rdfs:comment>The name of the shard group, used as cluster name in Distributed tables.</rdfs:comment>
    <rdfs:domain rdf:resource="http://example.org/onto/class/yandex_mdb_clickhouse_cluster"/>
    <rdfs:range rdf:resource="http://www.w3.org/2001/XMLSchema#string"/>
  </owl:DatatypeProperty>
  <owl:DatatypeProperty rdf:about="http://example.org/onto/prop/yandex_mdb_clickhouse_cluster_shard_names">
    <rdfs:label>shard_names</rdfs:label>
    <rdfs:comment>List of shards names that belong to the shard group.</rdfs:comment>
    <rdfs:domain rdf:resource="http://example.org/onto/class/yandex_mdb_clickhouse_cluster"/>
    <rdfs:range rdf:resource="http://www.w3.org/2001/XMLSchema#string"/>
  </owl:DatatypeProperty>
  <owl:DatatypeProperty rdf:about="http://example.org/onto/prop/yandex_mdb_clickhouse_cluster_create">
    <rdfs:label>create</rdfs:label>
    <rdfs:domain rdf:resource="http://example.org/onto/class/yandex_mdb_clickhouse_cluster"/>
    <rdfs:range rdf:resource="http://www.w3.org/2001/XMLSchema#string"/>
  </owl:DatatypeProperty>
  <owl:DatatypeProperty rdf:about="http://example.org/onto/prop/yandex_mdb_clickhouse_cluster_delete">
    <rdfs:label>delete</rdfs:label>
    <rdfs:domain rdf:resource="http://example.org/onto/class/yandex_mdb_clickhouse_cluster"/>
    <rdfs:range rdf:resource="http://www.w3.org/2001/XMLSchema#string"/>
  </owl:DatatypeProperty>
  <owl:DatatypeProperty rdf:about="http://example.org/onto/prop/yandex_mdb_clickhouse_cluster_update">
    <rdfs:label>update</rdfs:label>
    <rdfs:domain rdf:resource="http://example.org/onto/class/yandex_mdb_clickhouse_cluster"/>
    <rdfs:range rdf:resource="http://www.w3.org/2001/XMLSchema#string"/>
  </owl:DatatypeProperty>
  <owl:DatatypeProperty rdf:about="http://example.org/onto/prop/yandex_mdb_clickhouse_cluster_connection_manager">
    <rdfs:label>connection_manager</rdfs:label>
    <rdfs:comment>Connection Manager connection configuration. Filled in by the server automatically.</rdfs:comment>
    <rdfs:domain rdf:resource="http://example.org/onto/class/yandex_mdb_clickhouse_cluster"/>
    <rdfs:range rdf:resource="http://www.w3.org/2001/XMLSchema#string"/>
  </owl:DatatypeProperty>
  <owl:DatatypeProperty rdf:about="http://example.org/onto/prop/yandex_mdb_clickhouse_cluster_generate_password">
    <rdfs:label>generate_password</rdfs:label>
    <rdfs:comment>Generate password using Connection Manager. Allowed values: `true` or `false`. It's used only during user creation and is ignored during updating.

~> **Must specify either password or generate_password**.</rdfs:comment>
    <rdfs:domain rdf:resource="http://example.org/onto/class/yandex_mdb_clickhouse_cluster"/>
    <rdfs:range rdf:resource="http://www.w3.org/2001/XMLSchema#string"/>
  </owl:DatatypeProperty>
  <owl:DatatypeProperty rdf:about="http://example.org/onto/prop/yandex_mdb_clickhouse_cluster_name">
    <rdfs:label>name</rdfs:label>
    <rdfs:comment>The name of the user.</rdfs:comment>
    <rdfs:domain rdf:resource="http://example.org/onto/class/yandex_mdb_clickhouse_cluster"/>
    <rdfs:range rdf:resource="http://www.w3.org/2001/XMLSchema#string"/>
  </owl:DatatypeProperty>
  <owl:DatatypeProperty rdf:about="http://example.org/onto/prop/yandex_mdb_clickhouse_cluster_password">
    <rdfs:label>password</rdfs:label>
    <rdfs:comment>The password of the user.</rdfs:comment>
    <rdfs:domain rdf:resource="http://example.org/onto/class/yandex_mdb_clickhouse_cluster"/>
    <rdfs:range rdf:resource="http://www.w3.org/2001/XMLSchema#string"/>
  </owl:DatatypeProperty>
  <owl:DatatypeProperty rdf:about="http://example.org/onto/prop/yandex_mdb_clickhouse_cluster_database_name">
    <rdfs:label>database_name</rdfs:label>
    <rdfs:comment>The name of the database that the permission grants access to.</rdfs:comment>
    <rdfs:domain rdf:resource="http://example.org/onto/class/yandex_mdb_clickhouse_cluster"/>
    <rdfs:range rdf:resource="http://www.w3.org/2001/XMLSchema#string"/>
  </owl:DatatypeProperty>
  <owl:DatatypeProperty rdf:about="http://example.org/onto/prop/yandex_mdb_clickhouse_cluster_errors">
    <rdfs:label>errors</rdfs:label>
    <rdfs:comment>The number of queries that threw exception.</rdfs:comment>
    <rdfs:domain rdf:resource="http://example.org/onto/class/yandex_mdb_clickhouse_cluster"/>
    <rdfs:range rdf:resource="http://www.w3.org/2001/XMLSchema#string"/>
  </owl:DatatypeProperty>
  <owl:DatatypeProperty rdf:about="http://example.org/onto/prop/yandex_mdb_clickhouse_cluster_execution_time">
    <rdfs:label>execution_time</rdfs:label>
    <rdfs:comment>The total query execution time, in milliseconds (wall time).</rdfs:comment>
    <rdfs:domain rdf:resource="http://example.org/onto/class/yandex_mdb_clickhouse_cluster"/>
    <rdfs:range rdf:resource="http://www.w3.org/2001/XMLSchema#string"/>
  </owl:DatatypeProperty>
  <owl:DatatypeProperty rdf:about="http://example.org/onto/prop/yandex_mdb_clickhouse_cluster_interval_duration">
    <rdfs:label>interval_duration</rdfs:label>
    <rdfs:comment>Duration of interval for quota in milliseconds.</rdfs:comment>
    <rdfs:domain rdf:resource="http://example.org/onto/class/yandex_mdb_clickhouse_cluster"/>
    <rdfs:range rdf:resource="http://www.w3.org/2001/XMLSchema#string"/>
  </owl:DatatypeProperty>
  <owl:DatatypeProperty rdf:about="http://example.org/onto/prop/yandex_mdb_clickhouse_cluster_queries">
    <rdfs:label>queries</rdfs:label>
    <rdfs:comment>The total number of queries.</rdfs:comment>
    <rdfs:domain rdf:resource="http://example.org/onto/class/yandex_mdb_clickhouse_cluster"/>
    <rdfs:range rdf:resource="http://www.w3.org/2001/XMLSchema#string"/>
  </owl:DatatypeProperty>
  <owl:DatatypeProperty rdf:about="http://example.org/onto/prop/yandex_mdb_clickhouse_cluster_read_rows">
    <rdfs:label>read_rows</rdfs:label>
    <rdfs:comment>The total number of source rows read from tables for running the query, on all remote servers.</rdfs:comment>
    <rdfs:domain rdf:resource="http://example.org/onto/class/yandex_mdb_clickhouse_cluster"/>
    <rdfs:range rdf:resource="http://www.w3.org/2001/XMLSchema#string"/>
  </owl:DatatypeProperty>
  <owl:DatatypeProperty rdf:about="http://example.org/onto/prop/yandex_mdb_clickhouse_cluster_result_rows">
    <rdfs:label>result_rows</rdfs:label>
    <rdfs:comment>The total number of rows given as the result.</rdfs:comment>
    <rdfs:domain rdf:resource="http://example.org/onto/class/yandex_mdb_clickhouse_cluster"/>
    <rdfs:range rdf:resource="http://www.w3.org/2001/XMLSchema#string"/>
  </owl:DatatypeProperty>
  <owl:DatatypeProperty rdf:about="http://example.org/onto/prop/yandex_mdb_clickhouse_cluster_add_http_cors_header">
    <rdfs:label>add_http_cors_header</rdfs:label>
    <rdfs:comment>Include CORS headers in HTTP responses.</rdfs:comment>
    <rdfs:domain rdf:resource="http://example.org/onto/class/yandex_mdb_clickhouse_cluster"/>
    <rdfs:range rdf:resource="http://www.w3.org/2001/XMLSchema#string"/>
  </owl:DatatypeProperty>
  <owl:DatatypeProperty rdf:about="http://example.org/onto/prop/yandex_mdb_clickhouse_cluster_allow_ddl">
    <rdfs:label>allow_ddl</rdfs:label>
    <rdfs:comment>Allows or denies DDL queries.</rdfs:comment>
    <rdfs:domain rdf:resource="http://example.org/onto/class/yandex_mdb_clickhouse_cluster"/>
    <rdfs:range rdf:resource="http://www.w3.org/2001/XMLSchema#string"/>
  </owl:DatatypeProperty>
  <owl:DatatypeProperty rdf:about="http://example.org/onto/prop/yandex_mdb_clickhouse_cluster_allow_introspection_functions">
    <rdfs:label>allow_introspection_functions</rdfs:label>
    <rdfs:comment>Enables introspections functions for query profiling.</rdfs:comment>
    <rdfs:domain rdf:resource="http://example.org/onto/class/yandex_mdb_clickhouse_cluster"/>
    <rdfs:range rdf:resource="http://www.w3.org/2001/XMLSchema#string"/>
  </owl:DatatypeProperty>
  <owl:DatatypeProperty rdf:about="http://example.org/onto/prop/yandex_mdb_clickhouse_cluster_allow_suspicious_low_cardinality_types">
    <rdfs:label>allow_suspicious_low_cardinality_types</rdfs:label>
    <rdfs:comment>Allows specifying LowCardinality modifier for types of small fixed size (8 or less) in CREATE TABLE statements. Enabling this may increase merge times and memory consumption.</rdfs:comment>
    <rdfs:domain rdf:resource="http://example.org/onto/class/yandex_mdb_clickhouse_cluster"/>
    <rdfs:range rdf:resource="http://www.w3.org/2001/XMLSchema#string"/>
  </owl:DatatypeProperty>
  <owl:DatatypeProperty rdf:about="http://example.org/onto/prop/yandex_mdb_clickhouse_cluster_any_join_distinct_right_table_keys">
    <rdfs:label>any_join_distinct_right_table_keys</rdfs:label>
    <rdfs:comment>Enables legacy ClickHouse server behavior in ANY INNER|LEFT JOIN operations.</rdfs:comment>
    <rdfs:domain rdf:resource="http://example.org/onto/class/yandex_mdb_clickhouse_cluster"/>
    <rdfs:range rdf:resource="http://www.w3.org/2001/XMLSchema#string"/>
  </owl:DatatypeProperty>
  <owl:DatatypeProperty rdf:about="http://example.org/onto/prop/yandex_mdb_clickhouse_cluster_async_insert">
    <rdfs:label>async_insert</rdfs:label>
    <rdfs:comment>Enables asynchronous inserts. Disabled by default.</rdfs:comment>
    <rdfs:domain rdf:resource="http://example.org/onto/class/yandex_mdb_clickhouse_cluster"/>
    <rdfs:range rdf:resource="http://www.w3.org/2001/XMLSchema#string"/>
  </owl:DatatypeProperty>
  <owl:DatatypeProperty rdf:about="http://example.org/onto/prop/yandex_mdb_clickhouse_cluster_async_insert_busy_timeout">
    <rdfs:label>async_insert_busy_timeout</rdfs:label>
    <rdfs:comment>The maximum timeout in milliseconds since the first INSERT query before inserting collected data. If the parameter is set to 0, the timeout is disabled. Default value: 200.</rdfs:comment>
    <rdfs:domain rdf:resource="http://example.org/onto/class/yandex_mdb_clickhouse_cluster"/>
    <rdfs:range rdf:resource="http://www.w3.org/2001/XMLSchema#string"/>
  </owl:DatatypeProperty>
  <owl:DatatypeProperty rdf:about="http://example.org/onto/prop/yandex_mdb_clickhouse_cluster_async_insert_max_data_size">
    <rdfs:label>async_insert_max_data_size</rdfs:label>
    <rdfs:comment>The maximum size of the unparsed data in bytes collected per query before being inserted. If the parameter is set to 0, asynchronous insertions are disabled. Default value: 100000.</rdfs:comment>
    <rdfs:domain rdf:resource="http://example.org/onto/class/yandex_mdb_clickhouse_cluster"/>
    <rdfs:range rdf:resource="http://www.w3.org/2001/XMLSchema#string"/>
  </owl:DatatypeProperty>
  <owl:DatatypeProperty rdf:about="http://example.org/onto/prop/yandex_mdb_clickhouse_cluster_async_insert_stale_timeout">
    <rdfs:label>async_insert_stale_timeout</rdfs:label>
    <rdfs:comment>The maximum timeout in milliseconds since the last INSERT query before dumping collected data. If enabled, the settings prolongs the async_insert_busy_timeout with every INSERT query as long as async_insert_max_data_size is not exceeded.</rdfs:comment>
    <rdfs:domain rdf:resource="http://example.org/onto/class/yandex_mdb_clickhouse_cluster"/>
    <rdfs:range rdf:resource="http://www.w3.org/2001/XMLSchema#string"/>
  </owl:DatatypeProperty>
  <owl:DatatypeProperty rdf:about="http://example.org/onto/prop/yandex_mdb_clickhouse_cluster_async_insert_threads">
    <rdfs:label>async_insert_threads</rdfs:label>
    <rdfs:comment>The maximum number of threads for background data parsing and insertion. If the parameter is set to 0, asynchronous insertions are disabled. Default value: 16.</rdfs:comment>
    <rdfs:domain rdf:resource="http://example.org/onto/class/yandex_mdb_clickhouse_cluster"/>
    <rdfs:range rdf:resource="http://www.w3.org/2001/XMLSchema#string"/>
  </owl:DatatypeProperty>
  <owl:DatatypeProperty rdf:about="http://example.org/onto/prop/yandex_mdb_clickhouse_cluster_async_insert_use_adaptive_busy_timeout">
    <rdfs:label>async_insert_use_adaptive_busy_timeout</rdfs:label>
    <rdfs:comment>If it is set to true, use adaptive busy timeout for asynchronous inserts.</rdfs:comment>
    <rdfs:domain rdf:resource="http://example.org/onto/class/yandex_mdb_clickhouse_cluster"/>
    <rdfs:range rdf:resource="http://www.w3.org/2001/XMLSchema#string"/>
  </owl:DatatypeProperty>
  <owl:DatatypeProperty rdf:about="http://example.org/onto/prop/yandex_mdb_clickhouse_cluster_cancel_http_readonly_queries_on_client_close">
    <rdfs:label>cancel_http_readonly_queries_on_client_close</rdfs:label>
    <rdfs:comment>Cancels HTTP read-only queries (e.g. SELECT) when a client closes the connection without waiting for the response. Default value: false.</rdfs:comment>
    <rdfs:domain rdf:resource="http://example.org/onto/class/yandex_mdb_clickhouse_cluster"/>
    <rdfs:range rdf:resource="http://www.w3.org/2001/XMLSchema#string"/>
  </owl:DatatypeProperty>
  <owl:DatatypeProperty rdf:about="http://example.org/onto/prop/yandex_mdb_clickhouse_cluster_compile">
    <rdfs:label>compile</rdfs:label>
    <rdfs:comment>Enable compilation of queries.</rdfs:comment>
    <rdfs:domain rdf:resource="http://example.org/onto/class/yandex_mdb_clickhouse_cluster"/>
    <rdfs:range rdf:resource="http://www.w3.org/2001/XMLSchema#string"/>
  </owl:DatatypeProperty>
  <owl:DatatypeProperty rdf:about="http://example.org/onto/prop/yandex_mdb_clickhouse_cluster_compile_expressions">
    <rdfs:label>compile_expressions</rdfs:label>
    <rdfs:comment>Turn on expression compilation.</rdfs:comment>
    <rdfs:domain rdf:resource="http://example.org/onto/class/yandex_mdb_clickhouse_cluster"/>
    <rdfs:range rdf:resource="http://www.w3.org/2001/XMLSchema#string"/>
  </owl:DatatypeProperty>
  <owl:DatatypeProperty rdf:about="http://example.org/onto/prop/yandex_mdb_clickhouse_cluster_connect_timeout">
    <rdfs:label>connect_timeout</rdfs:label>
    <rdfs:comment>Connect timeout in milliseconds on the socket used for communicating with the client.</rdfs:comment>
    <rdfs:domain rdf:resource="http://example.org/onto/class/yandex_mdb_clickhouse_cluster"/>
    <rdfs:range rdf:resource="http://www.w3.org/2001/XMLSchema#string"/>
  </owl:DatatypeProperty>
  <owl:DatatypeProperty rdf:about="http://example.org/onto/prop/yandex_mdb_clickhouse_cluster_connect_timeout_with_failover">
    <rdfs:label>connect_timeout_with_failover</rdfs:label>
    <rdfs:comment>The timeout in milliseconds for connecting to a remote server for a Distributed table engine, if the ‘shard’ and ‘replica’ sections are used in the cluster definition. If unsuccessful, several attempts are made to connect to various replicas. Default value: 50.</rdfs:comment>
    <rdfs:domain rdf:resource="http://example.org/onto/class/yandex_mdb_clickhouse_cluster"/>
    <rdfs:range rdf:resource="http://www.w3.org/2001/XMLSchema#string"/>
  </owl:DatatypeProperty>
  <owl:DatatypeProperty rdf:about="http://example.org/onto/prop/yandex_mdb_clickhouse_cluster_count_distinct_implementation">
    <rdfs:label>count_distinct_implementation</rdfs:label>
    <rdfs:comment>Specifies which of the uniq* functions should be used to perform the COUNT(DISTINCT …) construction.</rdfs:comment>
    <rdfs:domain rdf:resource="http://example.org/onto/class/yandex_mdb_clickhouse_cluster"/>
    <rdfs:range rdf:resource="http://www.w3.org/2001/XMLSchema#string"/>
  </owl:DatatypeProperty>
  <owl:DatatypeProperty rdf:about="http://example.org/onto/prop/yandex_mdb_clickhouse_cluster_data_type_default_nullable">
    <rdfs:label>data_type_default_nullable</rdfs:label>
    <rdfs:comment>Allows data types without explicit modifiers NULL or NOT NULL in column definition will be Nullable.</rdfs:comment>
    <rdfs:domain rdf:resource="http://example.org/onto/class/yandex_mdb_clickhouse_cluster"/>
    <rdfs:range rdf:resource="http://www.w3.org/2001/XMLSchema#string"/>
  </owl:DatatypeProperty>
  <owl:DatatypeProperty rdf:about="http://example.org/onto/prop/yandex_mdb_clickhouse_cluster_date_time_input_format">
    <rdfs:label>date_time_input_format</rdfs:label>
    <rdfs:comment>Allows choosing a parser of the text representation of date and time, one of: `best_effort`, `basic`, `best_effort_us`. Default value: `basic`. Cloud default value: `best_effort`.</rdfs:comment>
    <rdfs:domain rdf:resource="http://example.org/onto/class/yandex_mdb_clickhouse_cluster"/>
    <rdfs:range rdf:resource="http://www.w3.org/2001/XMLSchema#string"/>
  </owl:DatatypeProperty>
  <owl:DatatypeProperty rdf:about="http://example.org/onto/prop/yandex_mdb_clickhouse_cluster_date_time_output_format">
    <rdfs:label>date_time_output_format</rdfs:label>
    <rdfs:comment>Allows choosing different output formats of the text representation of date and time, one of: `simple`, `iso`, `unix_timestamp`. Default value: `simple`.</rdfs:comment>
    <rdfs:domain rdf:resource="http://example.org/onto/class/yandex_mdb_clickhouse_cluster"/>
    <rdfs:range rdf:resource="http://www.w3.org/2001/XMLSchema#string"/>
  </owl:DatatypeProperty>
  <owl:DatatypeProperty rdf:about="http://example.org/onto/prop/yandex_mdb_clickhouse_cluster_deduplicate_blocks_in_dependent_materialized_views">
    <rdfs:label>deduplicate_blocks_in_dependent_materialized_views</rdfs:label>
    <rdfs:comment>Enables or disables the deduplication check for materialized views that receive data from `Replicated` tables.</rdfs:comment>
    <rdfs:domain rdf:resource="http://example.org/onto/class/yandex_mdb_clickhouse_cluster"/>
    <rdfs:range rdf:resource="http://www.w3.org/2001/XMLSchema#string"/>
  </owl:DatatypeProperty>
  <owl:DatatypeProperty rdf:about="http://example.org/onto/prop/yandex_mdb_clickhouse_cluster_distinct_overflow_mode">
    <rdfs:label>distinct_overflow_mode</rdfs:label>
    <rdfs:comment>Sets behavior on overflow when using DISTINCT. Possible values:
* `throw` - abort query execution, return an error.
* `break` - stop query execution, return partial result.</rdfs:comment>
    <rdfs:domain rdf:resource="http://example.org/onto/class/yandex_mdb_clickhouse_cluster"/>
    <rdfs:range rdf:resource="http://www.w3.org/2001/XMLSchema#string"/>
  </owl:DatatypeProperty>
  <owl:DatatypeProperty rdf:about="http://example.org/onto/prop/yandex_mdb_clickhouse_cluster_distributed_aggregation_memory_efficient">
    <rdfs:label>distributed_aggregation_memory_efficient</rdfs:label>
    <rdfs:comment>Determine the behavior of distributed subqueries.</rdfs:comment>
    <rdfs:domain rdf:resource="http://example.org/onto/class/yandex_mdb_clickhouse_cluster"/>
    <rdfs:range rdf:resource="http://www.w3.org/2001/XMLSchema#string"/>
  </owl:DatatypeProperty>
  <owl:DatatypeProperty rdf:about="http://example.org/onto/prop/yandex_mdb_clickhouse_cluster_distributed_ddl_task_timeout">
    <rdfs:label>distributed_ddl_task_timeout</rdfs:label>
    <rdfs:comment>Timeout for DDL queries, in milliseconds.</rdfs:comment>
    <rdfs:domain rdf:resource="http://example.org/onto/class/yandex_mdb_clickhouse_cluster"/>
    <rdfs:range rdf:resource="http://www.w3.org/2001/XMLSchema#string"/>
  </owl:DatatypeProperty>
  <owl:DatatypeProperty rdf:about="http://example.org/onto/prop/yandex_mdb_clickhouse_cluster_distributed_product_mode">
    <rdfs:label>distributed_product_mode</rdfs:label>
    <rdfs:comment>Changes the behavior of distributed subqueries.</rdfs:comment>
    <rdfs:domain rdf:resource="http://example.org/onto/class/yandex_mdb_clickhouse_cluster"/>
    <rdfs:range rdf:resource="http://www.w3.org/2001/XMLSchema#string"/>
  </owl:DatatypeProperty>
  <owl:DatatypeProperty rdf:about="http://example.org/onto/prop/yandex_mdb_clickhouse_cluster_do_not_merge_across_partitions_select_final">
    <rdfs:label>do_not_merge_across_partitions_select_final</rdfs:label>
    <rdfs:comment>Enable or disable independent processing of partitions for **SELECT** queries with **FINAL**.</rdfs:comment>
    <rdfs:domain rdf:resource="http://example.org/onto/class/yandex_mdb_clickhouse_cluster"/>
    <rdfs:range rdf:resource="http://www.w3.org/2001/XMLSchema#string"/>
  </owl:DatatypeProperty>
  <owl:DatatypeProperty rdf:about="http://example.org/onto/prop/yandex_mdb_clickhouse_cluster_empty_result_for_aggregation_by_empty_set">
    <rdfs:label>empty_result_for_aggregation_by_empty_set</rdfs:label>
    <rdfs:comment>Allows to return empty result.</rdfs:comment>
    <rdfs:domain rdf:resource="http://example.org/onto/class/yandex_mdb_clickhouse_cluster"/>
    <rdfs:range rdf:resource="http://www.w3.org/2001/XMLSchema#string"/>
  </owl:DatatypeProperty>
  <owl:DatatypeProperty rdf:about="http://example.org/onto/prop/yandex_mdb_clickhouse_cluster_enable_analyzer">
    <rdfs:label>enable_analyzer</rdfs:label>
    <rdfs:comment>Enable new query analyzer.</rdfs:comment>
    <rdfs:domain rdf:resource="http://example.org/onto/class/yandex_mdb_clickhouse_cluster"/>
    <rdfs:range rdf:resource="http://www.w3.org/2001/XMLSchema#string"/>
  </owl:DatatypeProperty>
  <owl:DatatypeProperty rdf:about="http://example.org/onto/prop/yandex_mdb_clickhouse_cluster_enable_http_compression">
    <rdfs:label>enable_http_compression</rdfs:label>
    <rdfs:comment>Enables or disables data compression in the response to an HTTP request.</rdfs:comment>
    <rdfs:domain rdf:resource="http://example.org/onto/class/yandex_mdb_clickhouse_cluster"/>
    <rdfs:range rdf:resource="http://www.w3.org/2001/XMLSchema#string"/>
  </owl:DatatypeProperty>
  <owl:DatatypeProperty rdf:about="http://example.org/onto/prop/yandex_mdb_clickhouse_cluster_enable_reads_from_query_cache">
    <rdfs:label>enable_reads_from_query_cache</rdfs:label>
    <rdfs:comment>If turned on, results of SELECT queries are retrieved from the query cache.</rdfs:comment>
    <rdfs:domain rdf:resource="http://example.org/onto/class/yandex_mdb_clickhouse_cluster"/>
    <rdfs:range rdf:resource="http://www.w3.org/2001/XMLSchema#string"/>
  </owl:DatatypeProperty>
  <owl:DatatypeProperty rdf:about="http://example.org/onto/prop/yandex_mdb_clickhouse_cluster_enable_writes_to_query_cache">
    <rdfs:label>enable_writes_to_query_cache</rdfs:label>
    <rdfs:comment>If turned on, results of SELECT queries are stored in the query cache.</rdfs:comment>
    <rdfs:domain rdf:resource="http://example.org/onto/class/yandex_mdb_clickhouse_cluster"/>
    <rdfs:range rdf:resource="http://www.w3.org/2001/XMLSchema#string"/>
  </owl:DatatypeProperty>
  <owl:DatatypeProperty rdf:about="http://example.org/onto/prop/yandex_mdb_clickhouse_cluster_fallback_to_stale_replicas_for_distributed_queries">
    <rdfs:label>fallback_to_stale_replicas_for_distributed_queries</rdfs:label>
    <rdfs:comment>Forces a query to an out-of-date replica if updated data is not available.</rdfs:comment>
    <rdfs:domain rdf:resource="http://example.org/onto/class/yandex_mdb_clickhouse_cluster"/>
    <rdfs:range rdf:resource="http://www.w3.org/2001/XMLSchema#string"/>
  </owl:DatatypeProperty>
  <owl:DatatypeProperty rdf:about="http://example.org/onto/prop/yandex_mdb_clickhouse_cluster_flatten_nested">
    <rdfs:label>flatten_nested</rdfs:label>
    <rdfs:comment>Sets the data format of a nested columns.</rdfs:comment>
    <rdfs:domain rdf:resource="http://example.org/onto/class/yandex_mdb_clickhouse_cluster"/>
    <rdfs:range rdf:resource="http://www.w3.org/2001/XMLSchema#string"/>
  </owl:DatatypeProperty>
  <owl:DatatypeProperty rdf:about="http://example.org/onto/prop/yandex_mdb_clickhouse_cluster_force_index_by_date">
    <rdfs:label>force_index_by_date</rdfs:label>
    <rdfs:comment>Disables query execution if the index can’t be used by date.</rdfs:comment>
    <rdfs:domain rdf:resource="http://example.org/onto/class/yandex_mdb_clickhouse_cluster"/>
    <rdfs:range rdf:resource="http://www.w3.org/2001/XMLSchema#string"/>
  </owl:DatatypeProperty>
  <owl:DatatypeProperty rdf:about="http://example.org/onto/prop/yandex_mdb_clickhouse_cluster_force_primary_key">
    <rdfs:label>force_primary_key</rdfs:label>
    <rdfs:comment>Disables query execution if indexing by the primary key is not possible.</rdfs:comment>
    <rdfs:domain rdf:resource="http://example.org/onto/class/yandex_mdb_clickhouse_cluster"/>
    <rdfs:range rdf:resource="http://www.w3.org/2001/XMLSchema#string"/>
  </owl:DatatypeProperty>
  <owl:DatatypeProperty rdf:about="http://example.org/onto/prop/yandex_mdb_clickhouse_cluster_format_avro_schema_registry_url">
    <rdfs:label>format_avro_schema_registry_url</rdfs:label>
    <rdfs:comment>Avro schema registry URL.</rdfs:comment>
    <rdfs:domain rdf:resource="http://example.org/onto/class/yandex_mdb_clickhouse_cluster"/>
    <rdfs:range rdf:resource="http://www.w3.org/2001/XMLSchema#string"/>
  </owl:DatatypeProperty>
  <owl:DatatypeProperty rdf:about="http://example.org/onto/prop/yandex_mdb_clickhouse_cluster_format_regexp">
    <rdfs:label>format_regexp</rdfs:label>
    <rdfs:comment>Regular expression (for Regexp format).</rdfs:comment>
    <rdfs:domain rdf:resource="http://example.org/onto/class/yandex_mdb_clickhouse_cluster"/>
    <rdfs:range rdf:resource="http://www.w3.org/2001/XMLSchema#string"/>
  </owl:DatatypeProperty>
  <owl:DatatypeProperty rdf:about="http://example.org/onto/prop/yandex_mdb_clickhouse_cluster_format_regexp_skip_unmatched">
    <rdfs:label>format_regexp_skip_unmatched</rdfs:label>
    <rdfs:comment>Skip lines unmatched by regular expression.</rdfs:comment>
    <rdfs:domain rdf:resource="http://example.org/onto/class/yandex_mdb_clickhouse_cluster"/>
    <rdfs:range rdf:resource="http://www.w3.org/2001/XMLSchema#string"/>
  </owl:DatatypeProperty>
  <owl:DatatypeProperty rdf:about="http://example.org/onto/prop/yandex_mdb_clickhouse_cluster_group_by_overflow_mode">
    <rdfs:label>group_by_overflow_mode</rdfs:label>
    <rdfs:comment>Sets behavior on overflow while GROUP BY operation. Possible values:
* `throw` - abort query execution, return an error.
* `break` - stop query execution, return partial result.
* `any` - perform approximate GROUP BY operation by continuing aggregation for the keys that got into the set, but don’t add new keys to the set.</rdfs:comment>
    <rdfs:domain rdf:resource="http://example.org/onto/class/yandex_mdb_clickhouse_cluster"/>
    <rdfs:range rdf:resource="http://www.w3.org/2001/XMLSchema#string"/>
  </owl:DatatypeProperty>
  <owl:DatatypeProperty rdf:about="http://example.org/onto/prop/yandex_mdb_clickhouse_cluster_group_by_two_level_threshold">
    <rdfs:label>group_by_two_level_threshold</rdfs:label>
    <rdfs:comment>Sets the threshold of the number of keys, after that the two-level aggregation should be used.</rdfs:comment>
    <rdfs:domain rdf:resource="http://example.org/onto/class/yandex_mdb_clickhouse_cluster"/>
    <rdfs:range rdf:resource="http://www.w3.org/2001/XMLSchema#string"/>
  </owl:DatatypeProperty>
  <owl:DatatypeProperty rdf:about="http://example.org/onto/prop/yandex_mdb_clickhouse_cluster_group_by_two_level_threshold_bytes">
    <rdfs:label>group_by_two_level_threshold_bytes</rdfs:label>
    <rdfs:comment>Sets the threshold of the number of bytes, after that the two-level aggregation should be used.</rdfs:comment>
    <rdfs:domain rdf:resource="http://example.org/onto/class/yandex_mdb_clickhouse_cluster"/>
    <rdfs:range rdf:resource="http://www.w3.org/2001/XMLSchema#string"/>
  </owl:DatatypeProperty>
  <owl:DatatypeProperty rdf:about="http://example.org/onto/prop/yandex_mdb_clickhouse_cluster_hedged_connection_timeout_ms">
    <rdfs:label>hedged_connection_timeout_ms</rdfs:label>
    <rdfs:comment>Connection timeout for establishing connection with replica for Hedged requests. Default value: 50 milliseconds.</rdfs:comment>
    <rdfs:domain rdf:resource="http://example.org/onto/class/yandex_mdb_clickhouse_cluster"/>
    <rdfs:range rdf:resource="http://www.w3.org/2001/XMLSchema#string"/>
  </owl:DatatypeProperty>
  <owl:DatatypeProperty rdf:about="http://example.org/onto/prop/yandex_mdb_clickhouse_cluster_http_connection_timeout">
    <rdfs:label>http_connection_timeout</rdfs:label>
    <rdfs:comment>Timeout for HTTP connection in milliseconds.</rdfs:comment>
    <rdfs:domain rdf:resource="http://example.org/onto/class/yandex_mdb_clickhouse_cluster"/>
    <rdfs:range rdf:resource="http://www.w3.org/2001/XMLSchema#string"/>
  </owl:DatatypeProperty>
  <owl:DatatypeProperty rdf:about="http://example.org/onto/prop/yandex_mdb_clickhouse_cluster_http_headers_progress_interval">
    <rdfs:label>http_headers_progress_interval</rdfs:label>
    <rdfs:comment>Sets minimal interval between notifications about request process in HTTP header X-ClickHouse-Progress.</rdfs:comment>
    <rdfs:domain rdf:resource="http://example.org/onto/class/yandex_mdb_clickhouse_cluster"/>
    <rdfs:range rdf:resource="http://www.w3.org/2001/XMLSchema#string"/>
  </owl:DatatypeProperty>
  <owl:DatatypeProperty rdf:about="http://example.org/onto/prop/yandex_mdb_clickhouse_cluster_http_max_field_name_size">
    <rdfs:label>http_max_field_name_size</rdfs:label>
    <rdfs:comment>Maximum length of field name in HTTP header.</rdfs:comment>
    <rdfs:domain rdf:resource="http://example.org/onto/class/yandex_mdb_clickhouse_cluster"/>
    <rdfs:range rdf:resource="http://www.w3.org/2001/XMLSchema#string"/>
  </owl:DatatypeProperty>
  <owl:DatatypeProperty rdf:about="http://example.org/onto/prop/yandex_mdb_clickhouse_cluster_http_max_field_value_size">
    <rdfs:label>http_max_field_value_size</rdfs:label>
    <rdfs:comment>Maximum length of field value in HTTP header.</rdfs:comment>
    <rdfs:domain rdf:resource="http://example.org/onto/class/yandex_mdb_clickhouse_cluster"/>
    <rdfs:range rdf:resource="http://www.w3.org/2001/XMLSchema#string"/>
  </owl:DatatypeProperty>
  <owl:DatatypeProperty rdf:about="http://example.org/onto/prop/yandex_mdb_clickhouse_cluster_http_receive_timeout">
    <rdfs:label>http_receive_timeout</rdfs:label>
    <rdfs:comment>Timeout for HTTP connection in milliseconds.</rdfs:comment>
    <rdfs:domain rdf:resource="http://example.org/onto/class/yandex_mdb_clickhouse_cluster"/>
    <rdfs:range rdf:resource="http://www.w3.org/2001/XMLSchema#string"/>
  </owl:DatatypeProperty>
  <owl:DatatypeProperty rdf:about="http://example.org/onto/prop/yandex_mdb_clickhouse_cluster_http_send_timeout">
    <rdfs:label>http_send_timeout</rdfs:label>
    <rdfs:comment>Timeout for HTTP connection in milliseconds.</rdfs:comment>
    <rdfs:domain rdf:resource="http://example.org/onto/class/yandex_mdb_clickhouse_cluster"/>
    <rdfs:range rdf:resource="http://www.w3.org/2001/XMLSchema#string"/>
  </owl:DatatypeProperty>
  <owl:DatatypeProperty rdf:about="http://example.org/onto/prop/yandex_mdb_clickhouse_cluster_idle_connection_timeout">
    <rdfs:label>idle_connection_timeout</rdfs:label>
    <rdfs:comment>Timeout to close idle TCP connections after specified number of seconds. Default value: 3600 seconds.</rdfs:comment>
    <rdfs:domain rdf:resource="http://example.org/onto/class/yandex_mdb_clickhouse_cluster"/>
    <rdfs:range rdf:resource="http://www.w3.org/2001/XMLSchema#string"/>
  </owl:DatatypeProperty>
  <owl:DatatypeProperty rdf:about="http://example.org/onto/prop/yandex_mdb_clickhouse_cluster_ignore_materialized_views_with_dropped_target_table">
    <rdfs:label>ignore_materialized_views_with_dropped_target_table</rdfs:label>
    <rdfs:comment>Ignore materialized views with dropped target table during pushing to views.</rdfs:comment>
    <rdfs:domain rdf:resource="http://example.org/onto/class/yandex_mdb_clickhouse_cluster"/>
    <rdfs:range rdf:resource="http://www.w3.org/2001/XMLSchema#string"/>
  </owl:DatatypeProperty>
  <owl:DatatypeProperty rdf:about="http://example.org/onto/prop/yandex_mdb_clickhouse_cluster_input_format_defaults_for_omitted_fields">
    <rdfs:label>input_format_defaults_for_omitted_fields</rdfs:label>
    <rdfs:comment>When performing INSERT queries, replace omitted input column values with default values of the respective columns.</rdfs:comment>
    <rdfs:domain rdf:resource="http://example.org/onto/class/yandex_mdb_clickhouse_cluster"/>
    <rdfs:range rdf:resource="http://www.w3.org/2001/XMLSchema#string"/>
  </owl:DatatypeProperty>
  <owl:DatatypeProperty rdf:about="http://example.org/onto/prop/yandex_mdb_clickhouse_cluster_input_format_import_nested_json">
    <rdfs:label>input_format_import_nested_json</rdfs:label>
    <rdfs:comment>Enables or disables the insertion of JSON data with nested objects.</rdfs:comment>
    <rdfs:domain rdf:resource="http://example.org/onto/class/yandex_mdb_clickhouse_cluster"/>
    <rdfs:range rdf:resource="http://www.w3.org/2001/XMLSchema#string"/>
  </owl:DatatypeProperty>
  <owl:DatatypeProperty rdf:about="http://example.org/onto/prop/yandex_mdb_clickhouse_cluster_input_format_null_as_default">
    <rdfs:label>input_format_null_as_default</rdfs:label>
    <rdfs:comment>Enables or disables the initialization of NULL fields with default values, if data type of these fields is not nullable.</rdfs:comment>
    <rdfs:domain rdf:resource="http://example.org/onto/class/yandex_mdb_clickhouse_cluster"/>
    <rdfs:range rdf:resource="http://www.w3.org/2001/XMLSchema#string"/>
  </owl:DatatypeProperty>
  <owl:DatatypeProperty rdf:about="http://example.org/onto/prop/yandex_mdb_clickhouse_cluster_input_format_parallel_parsing">
    <rdfs:label>input_format_parallel_parsing</rdfs:label>
    <rdfs:comment>Enables or disables order-preserving parallel parsing of data formats. Supported only for TSV, TKSV, CSV and JSONEachRow formats.</rdfs:comment>
    <rdfs:domain rdf:resource="http://example.org/onto/class/yandex_mdb_clickhouse_cluster"/>
    <rdfs:range rdf:resource="http://www.w3.org/2001/XMLSchema#string"/>
  </owl:DatatypeProperty>
  <owl:DatatypeProperty rdf:about="http://example.org/onto/prop/yandex_mdb_clickhouse_cluster_input_format_values_interpret_expressions">
    <rdfs:label>input_format_values_interpret_expressions</rdfs:label>
    <rdfs:comment>Enables or disables the full SQL parser if the fast stream parser can’t parse the data.</rdfs:comment>
    <rdfs:domain rdf:resource="http://example.org/onto/class/yandex_mdb_clickhouse_cluster"/>
    <rdfs:range rdf:resource="http://www.w3.org/2001/XMLSchema#string"/>
  </owl:DatatypeProperty>
  <owl:DatatypeProperty rdf:about="http://example.org/onto/prop/yandex_mdb_clickhouse_cluster_input_format_with_names_use_header">
    <rdfs:label>input_format_with_names_use_header</rdfs:label>
    <rdfs:comment>Enables or disables checking the column order when inserting data.</rdfs:comment>
    <rdfs:domain rdf:resource="http://example.org/onto/class/yandex_mdb_clickhouse_cluster"/>
    <rdfs:range rdf:resource="http://www.w3.org/2001/XMLSchema#string"/>
  </owl:DatatypeProperty>
  <owl:DatatypeProperty rdf:about="http://example.org/onto/prop/yandex_mdb_clickhouse_cluster_insert_keeper_max_retries">
    <rdfs:label>insert_keeper_max_retries</rdfs:label>
    <rdfs:comment>The setting sets the maximum number of retries for ClickHouse Keeper (or ZooKeeper) requests during insert into replicated MergeTree. Only Keeper requests which failed due to network error, Keeper session timeout, or request timeout are considered for retries.</rdfs:comment>
    <rdfs:domain rdf:resource="http://example.org/onto/class/yandex_mdb_clickhouse_cluster"/>
    <rdfs:range rdf:resource="http://www.w3.org/2001/XMLSchema#string"/>
  </owl:DatatypeProperty>
  <owl:DatatypeProperty rdf:about="http://example.org/onto/prop/yandex_mdb_clickhouse_cluster_insert_null_as_default">
    <rdfs:label>insert_null_as_default</rdfs:label>
    <rdfs:comment>Enables the insertion of default values instead of NULL into columns with not nullable data type. Default value: true.</rdfs:comment>
    <rdfs:domain rdf:resource="http://example.org/onto/class/yandex_mdb_clickhouse_cluster"/>
    <rdfs:range rdf:resource="http://www.w3.org/2001/XMLSchema#string"/>
  </owl:DatatypeProperty>
  <owl:DatatypeProperty rdf:about="http://example.org/onto/prop/yandex_mdb_clickhouse_cluster_insert_quorum">
    <rdfs:label>insert_quorum</rdfs:label>
    <rdfs:comment>Enables the quorum writes.</rdfs:comment>
    <rdfs:domain rdf:resource="http://example.org/onto/class/yandex_mdb_clickhouse_cluster"/>
    <rdfs:range rdf:resource="http://www.w3.org/2001/XMLSchema#string"/>
  </owl:DatatypeProperty>
  <owl:DatatypeProperty rdf:about="http://example.org/onto/prop/yandex_mdb_clickhouse_cluster_insert_quorum_parallel">
    <rdfs:label>insert_quorum_parallel</rdfs:label>
    <rdfs:comment>Enables or disables parallelism for quorum INSERT queries.</rdfs:comment>
    <rdfs:domain rdf:resource="http://example.org/onto/class/yandex_mdb_clickhouse_cluster"/>
    <rdfs:range rdf:resource="http://www.w3.org/2001/XMLSchema#string"/>
  </owl:DatatypeProperty>
  <owl:DatatypeProperty rdf:about="http://example.org/onto/prop/yandex_mdb_clickhouse_cluster_insert_quorum_timeout">
    <rdfs:label>insert_quorum_timeout</rdfs:label>
    <rdfs:comment>Write to a quorum timeout in milliseconds.</rdfs:comment>
    <rdfs:domain rdf:resource="http://example.org/onto/class/yandex_mdb_clickhouse_cluster"/>
    <rdfs:range rdf:resource="http://www.w3.org/2001/XMLSchema#string"/>
  </owl:DatatypeProperty>
  <owl:DatatypeProperty rdf:about="http://example.org/onto/prop/yandex_mdb_clickhouse_cluster_join_algorithm">
    <rdfs:label>join_algorithm</rdfs:label>
    <rdfs:comment>Specifies which JOIN algorithm is used. Possible values:
* `hash` - hash join algorithm is used. The most generic implementation that supports all combinations of kind and strictness and multiple join keys that are combined with OR in the JOIN ON section.
* `parallel_hash` - a variation of hash join that splits the data into buckets and builds several hash tables instead of one concurrently to speed up this process.
* `partial_merge` - a variation of the sort-merge algorithm, where only the right table is fully sorted.
* `direct` - this algorithm can be applied when the storage for the right table supports key-value requests.
* `auto` - when set to auto, hash join is tried first, and the algorithm is switched on the fly to another algorithm if the memory limit is violated.
* `full_sorting_merge` - sort-merge algorithm with full sorting joined tables before joining.
* `prefer_partial_merge` - clickHouse always tries to use partial_merge join if possible, otherwise, it uses hash. Deprecated, same as partial_merge,hash.</rdfs:comment>
    <rdfs:domain rdf:resource="http://example.org/onto/class/yandex_mdb_clickhouse_cluster"/>
    <rdfs:range rdf:resource="http://www.w3.org/2001/XMLSchema#string"/>
  </owl:DatatypeProperty>
  <owl:DatatypeProperty rdf:about="http://example.org/onto/prop/yandex_mdb_clickhouse_cluster_join_overflow_mode">
    <rdfs:label>join_overflow_mode</rdfs:label>
    <rdfs:comment>Sets behavior on overflow in JOIN. Possible values:
* `throw` - abort query execution, return an error.
* `break` - stop query execution, return partial result.</rdfs:comment>
    <rdfs:domain rdf:resource="http://example.org/onto/class/yandex_mdb_clickhouse_cluster"/>
    <rdfs:range rdf:resource="http://www.w3.org/2001/XMLSchema#string"/>
  </owl:DatatypeProperty>
  <owl:DatatypeProperty rdf:about="http://example.org/onto/prop/yandex_mdb_clickhouse_cluster_join_use_nulls">
    <rdfs:label>join_use_nulls</rdfs:label>
    <rdfs:comment>Sets the type of JOIN behavior. When merging tables, empty cells may appear. ClickHouse fills them differently based on this setting.</rdfs:comment>
    <rdfs:domain rdf:resource="http://example.org/onto/class/yandex_mdb_clickhouse_cluster"/>
    <rdfs:range rdf:resource="http://www.w3.org/2001/XMLSchema#string"/>
  </owl:DatatypeProperty>
  <owl:DatatypeProperty rdf:about="http://example.org/onto/prop/yandex_mdb_clickhouse_cluster_joined_subquery_requires_alias">
    <rdfs:label>joined_subquery_requires_alias</rdfs:label>
    <rdfs:comment>Require aliases for subselects and table functions in FROM that more than one table is present.</rdfs:comment>
    <rdfs:domain rdf:resource="http://example.org/onto/class/yandex_mdb_clickhouse_cluster"/>
    <rdfs:range rdf:resource="http://www.w3.org/2001/XMLSchema#string"/>
  </owl:DatatypeProperty>
  <owl:DatatypeProperty rdf:about="http://example.org/onto/prop/yandex_mdb_clickhouse_cluster_load_balancing">
    <rdfs:label>load_balancing</rdfs:label>
    <rdfs:comment>Specifies the algorithm of replicas selection that is used for distributed query processing, one of: random, nearest_hostname, in_order, first_or_random, round_robin. Default value: random.</rdfs:comment>
    <rdfs:domain rdf:resource="http://example.org/onto/class/yandex_mdb_clickhouse_cluster"/>
    <rdfs:range rdf:resource="http://www.w3.org/2001/XMLSchema#string"/>
  </owl:DatatypeProperty>
  <owl:DatatypeProperty rdf:about="http://example.org/onto/prop/yandex_mdb_clickhouse_cluster_local_filesystem_read_method">
    <rdfs:label>local_filesystem_read_method</rdfs:label>
    <rdfs:comment>Method of reading data from local filesystem. Possible values:
* `read` - abort query execution, return an error.
* `pread` - abort query execution, return an error.
* `pread_threadpool` - stop query execution, return partial result. If the parameter is set to 0 (default), no hops is allowed.</rdfs:comment>
    <rdfs:domain rdf:resource="http://example.org/onto/class/yandex_mdb_clickhouse_cluster"/>
    <rdfs:range rdf:resource="http://www.w3.org/2001/XMLSchema#string"/>
  </owl:DatatypeProperty>
  <owl:DatatypeProperty rdf:about="http://example.org/onto/prop/yandex_mdb_clickhouse_cluster_log_processors_profiles">
    <rdfs:label>log_processors_profiles</rdfs:label>
    <rdfs:comment>Enabled or disable logging of processors level profiling data to the the system.log_processors_profiles table.</rdfs:comment>
    <rdfs:domain rdf:resource="http://example.org/onto/class/yandex_mdb_clickhouse_cluster"/>
    <rdfs:range rdf:resource="http://www.w3.org/2001/XMLSchema#string"/>
  </owl:DatatypeProperty>
  <owl:DatatypeProperty rdf:about="http://example.org/onto/prop/yandex_mdb_clickhouse_cluster_log_queries_probability">
    <rdfs:label>log_queries_probability</rdfs:label>
    <rdfs:comment>Log queries with the specified probability.</rdfs:comment>
    <rdfs:domain rdf:resource="http://example.org/onto/class/yandex_mdb_clickhouse_cluster"/>
    <rdfs:range rdf:resource="http://www.w3.org/2001/XMLSchema#string"/>
  </owl:DatatypeProperty>
  <owl:DatatypeProperty rdf:about="http://example.org/onto/prop/yandex_mdb_clickhouse_cluster_log_query_threads">
    <rdfs:label>log_query_threads</rdfs:label>
    <rdfs:comment>Setting up query threads logging. Query threads log into the system.query_thread_log table. This setting has effect only when log_queries is true. Queries’ threads run by ClickHouse with this setup are logged according to the rules in the query_thread_log server configuration parameter. Default value: `true`.</rdfs:comment>
    <rdfs:domain rdf:resource="http://example.org/onto/class/yandex_mdb_clickhouse_cluster"/>
    <rdfs:range rdf:resource="http://www.w3.org/2001/XMLSchema#string"/>
  </owl:DatatypeProperty>
  <owl:DatatypeProperty rdf:about="http://example.org/onto/prop/yandex_mdb_clickhouse_cluster_log_query_views">
    <rdfs:label>log_query_views</rdfs:label>
    <rdfs:comment>Enables or disables query views logging to the the system.query_views_log table.</rdfs:comment>
    <rdfs:domain rdf:resource="http://example.org/onto/class/yandex_mdb_clickhouse_cluster"/>
    <rdfs:range rdf:resource="http://www.w3.org/2001/XMLSchema#string"/>
  </owl:DatatypeProperty>
  <owl:DatatypeProperty rdf:about="http://example.org/onto/prop/yandex_mdb_clickhouse_cluster_low_cardinality_allow_in_native_format">
    <rdfs:label>low_cardinality_allow_in_native_format</rdfs:label>
    <rdfs:comment>Allows or restricts using the LowCardinality data type with the Native format.</rdfs:comment>
    <rdfs:domain rdf:resource="http://example.org/onto/class/yandex_mdb_clickhouse_cluster"/>
    <rdfs:range rdf:resource="http://www.w3.org/2001/XMLSchema#string"/>
  </owl:DatatypeProperty>
  <owl:DatatypeProperty rdf:about="http://example.org/onto/prop/yandex_mdb_clickhouse_cluster_max_ast_depth">
    <rdfs:label>max_ast_depth</rdfs:label>
    <rdfs:comment>Maximum abstract syntax tree depth.</rdfs:comment>
    <rdfs:domain rdf:resource="http://example.org/onto/class/yandex_mdb_clickhouse_cluster"/>
    <rdfs:range rdf:resource="http://www.w3.org/2001/XMLSchema#string"/>
  </owl:DatatypeProperty>
  <owl:DatatypeProperty rdf:about="http://example.org/onto/prop/yandex_mdb_clickhouse_cluster_max_ast_elements">
    <rdfs:label>max_ast_elements</rdfs:label>
    <rdfs:comment>Maximum abstract syntax tree elements.</rdfs:comment>
    <rdfs:domain rdf:resource="http://example.org/onto/class/yandex_mdb_clickhouse_cluster"/>
    <rdfs:range rdf:resource="http://www.w3.org/2001/XMLSchema#string"/>
  </owl:DatatypeProperty>
  <owl:DatatypeProperty rdf:about="http://example.org/onto/prop/yandex_mdb_clickhouse_cluster_max_block_size">
    <rdfs:label>max_block_size</rdfs:label>
    <rdfs:comment>A recommendation for what size of the block (in a count of rows) to load from tables.</rdfs:comment>
    <rdfs:domain rdf:resource="http://example.org/onto/class/yandex_mdb_clickhouse_cluster"/>
    <rdfs:range rdf:resource="http://www.w3.org/2001/XMLSchema#string"/>
  </owl:DatatypeProperty>
  <owl:DatatypeProperty rdf:about="http://example.org/onto/prop/yandex_mdb_clickhouse_cluster_max_bytes_before_external_group_by">
    <rdfs:label>max_bytes_before_external_group_by</rdfs:label>
    <rdfs:comment>Limit in bytes for using memory for GROUP BY before using swap on disk.</rdfs:comment>
    <rdfs:domain rdf:resource="http://example.org/onto/class/yandex_mdb_clickhouse_cluster"/>
    <rdfs:range rdf:resource="http://www.w3.org/2001/XMLSchema#string"/>
  </owl:DatatypeProperty>
  <owl:DatatypeProperty rdf:about="http://example.org/onto/prop/yandex_mdb_clickhouse_cluster_max_bytes_before_external_sort">
    <rdfs:label>max_bytes_before_external_sort</rdfs:label>
    <rdfs:comment>This setting is equivalent of the max_bytes_before_external_group_by setting, except for it is for sort operation (ORDER BY), not aggregation.</rdfs:comment>
    <rdfs:domain rdf:resource="http://example.org/onto/class/yandex_mdb_clickhouse_cluster"/>
    <rdfs:range rdf:resource="http://www.w3.org/2001/XMLSchema#string"/>
  </owl:DatatypeProperty>
  <owl:DatatypeProperty rdf:about="http://example.org/onto/prop/yandex_mdb_clickhouse_cluster_max_bytes_in_distinct">
    <rdfs:label>max_bytes_in_distinct</rdfs:label>
    <rdfs:comment>Limits the maximum size of a hash table in bytes (uncompressed data) when using DISTINCT.</rdfs:comment>
    <rdfs:domain rdf:resource="http://example.org/onto/class/yandex_mdb_clickhouse_cluster"/>
    <rdfs:range rdf:resource="http://www.w3.org/2001/XMLSchema#string"/>
  </owl:DatatypeProperty>
  <owl:DatatypeProperty rdf:about="http://example.org/onto/prop/yandex_mdb_clickhouse_cluster_max_bytes_in_join">
    <rdfs:label>max_bytes_in_join</rdfs:label>
    <rdfs:comment>Limit on maximum size of the hash table for JOIN, in bytes.</rdfs:comment>
    <rdfs:domain rdf:resource="http://example.org/onto/class/yandex_mdb_clickhouse_cluster"/>
    <rdfs:range rdf:resource="http://www.w3.org/2001/XMLSchema#string"/>
  </owl:DatatypeProperty>
  <owl:DatatypeProperty rdf:about="http://example.org/onto/prop/yandex_mdb_clickhouse_cluster_max_bytes_in_set">
    <rdfs:label>max_bytes_in_set</rdfs:label>
    <rdfs:comment>Limit on the number of bytes in the set resulting from the execution of the IN section.</rdfs:comment>
    <rdfs:domain rdf:resource="http://example.org/onto/class/yandex_mdb_clickhouse_cluster"/>
    <rdfs:range rdf:resource="http://www.w3.org/2001/XMLSchema#string"/>
  </owl:DatatypeProperty>
  <owl:DatatypeProperty rdf:about="http://example.org/onto/prop/yandex_mdb_clickhouse_cluster_max_bytes_to_read">
    <rdfs:label>max_bytes_to_read</rdfs:label>
    <rdfs:comment>Limits the maximum number of bytes (uncompressed data) that can be read from a table when running a query.</rdfs:comment>
    <rdfs:domain rdf:resource="http://example.org/onto/class/yandex_mdb_clickhouse_cluster"/>
    <rdfs:range rdf:resource="http://www.w3.org/2001/XMLSchema#string"/>
  </owl:DatatypeProperty>
  <owl:DatatypeProperty rdf:about="http://example.org/onto/prop/yandex_mdb_clickhouse_cluster_max_bytes_to_sort">
    <rdfs:label>max_bytes_to_sort</rdfs:label>
    <rdfs:comment>Limits the maximum number of bytes (uncompressed data) that can be read from a table for sorting.</rdfs:comment>
    <rdfs:domain rdf:resource="http://example.org/onto/class/yandex_mdb_clickhouse_cluster"/>
    <rdfs:range rdf:resource="http://www.w3.org/2001/XMLSchema#string"/>
  </owl:DatatypeProperty>
  <owl:DatatypeProperty rdf:about="http://example.org/onto/prop/yandex_mdb_clickhouse_cluster_max_bytes_to_transfer">
    <rdfs:label>max_bytes_to_transfer</rdfs:label>
    <rdfs:comment>Limits the maximum number of bytes (uncompressed data) that can be passed to a remote server or saved in a temporary table when using GLOBAL IN.</rdfs:comment>
    <rdfs:domain rdf:resource="http://example.org/onto/class/yandex_mdb_clickhouse_cluster"/>
    <rdfs:range rdf:resource="http://www.w3.org/2001/XMLSchema#string"/>
  </owl:DatatypeProperty>
  <owl:DatatypeProperty rdf:about="http://example.org/onto/prop/yandex_mdb_clickhouse_cluster_max_columns_to_read">
    <rdfs:label>max_columns_to_read</rdfs:label>
    <rdfs:comment>Limits the maximum number of columns that can be read from a table in a single query.</rdfs:comment>
    <rdfs:domain rdf:resource="http://example.org/onto/class/yandex_mdb_clickhouse_cluster"/>
    <rdfs:range rdf:resource="http://www.w3.org/2001/XMLSchema#string"/>
  </owl:DatatypeProperty>
  <owl:DatatypeProperty rdf:about="http://example.org/onto/prop/yandex_mdb_clickhouse_cluster_max_concurrent_queries_for_user">
    <rdfs:label>max_concurrent_queries_for_user</rdfs:label>
    <rdfs:comment>The maximum number of concurrent requests per user. Default value: 0 (no limit).</rdfs:comment>
    <rdfs:domain rdf:resource="http://example.org/onto/class/yandex_mdb_clickhouse_cluster"/>
    <rdfs:range rdf:resource="http://www.w3.org/2001/XMLSchema#string"/>
  </owl:DatatypeProperty>
  <owl:DatatypeProperty rdf:about="http://example.org/onto/prop/yandex_mdb_clickhouse_cluster_max_execution_time">
    <rdfs:label>max_execution_time</rdfs:label>
    <rdfs:comment>Limits the maximum query execution time in milliseconds.</rdfs:comment>
    <rdfs:domain rdf:resource="http://example.org/onto/class/yandex_mdb_clickhouse_cluster"/>
    <rdfs:range rdf:resource="http://www.w3.org/2001/XMLSchema#string"/>
  </owl:DatatypeProperty>
  <owl:DatatypeProperty rdf:about="http://example.org/onto/prop/yandex_mdb_clickhouse_cluster_max_expanded_ast_elements">
    <rdfs:label>max_expanded_ast_elements</rdfs:label>
    <rdfs:comment>Maximum abstract syntax tree depth after after expansion of aliases.</rdfs:comment>
    <rdfs:domain rdf:resource="http://example.org/onto/class/yandex_mdb_clickhouse_cluster"/>
    <rdfs:range rdf:resource="http://www.w3.org/2001/XMLSchema#string"/>
  </owl:DatatypeProperty>
  <owl:DatatypeProperty rdf:about="http://example.org/onto/prop/yandex_mdb_clickhouse_cluster_max_final_threads">
    <rdfs:label>max_final_threads</rdfs:label>
    <rdfs:comment>Sets the maximum number of parallel threads for the SELECT query data read phase with the FINAL modifier.</rdfs:comment>
    <rdfs:domain rdf:resource="http://example.org/onto/class/yandex_mdb_clickhouse_cluster"/>
    <rdfs:range rdf:resource="http://www.w3.org/2001/XMLSchema#string"/>
  </owl:DatatypeProperty>
  <owl:DatatypeProperty rdf:about="http://example.org/onto/prop/yandex_mdb_clickhouse_cluster_max_http_get_redirects">
    <rdfs:label>max_http_get_redirects</rdfs:label>
    <rdfs:comment>Limits the maximum number of HTTP GET redirect hops for URL-engine tables.</rdfs:comment>
    <rdfs:domain rdf:resource="http://example.org/onto/class/yandex_mdb_clickhouse_cluster"/>
    <rdfs:range rdf:resource="http://www.w3.org/2001/XMLSchema#string"/>
  </owl:DatatypeProperty>
  <owl:DatatypeProperty rdf:about="http://example.org/onto/prop/yandex_mdb_clickhouse_cluster_max_insert_block_size">
    <rdfs:label>max_insert_block_size</rdfs:label>
    <rdfs:comment>The size of blocks (in a count of rows) to form for insertion into a table.</rdfs:comment>
    <rdfs:domain rdf:resource="http://example.org/onto/class/yandex_mdb_clickhouse_cluster"/>
    <rdfs:range rdf:resource="http://www.w3.org/2001/XMLSchema#string"/>
  </owl:DatatypeProperty>
  <owl:DatatypeProperty rdf:about="http://example.org/onto/prop/yandex_mdb_clickhouse_cluster_max_insert_threads">
    <rdfs:label>max_insert_threads</rdfs:label>
    <rdfs:comment>The maximum number of threads to execute the INSERT SELECT query. Default value: 0.</rdfs:comment>
    <rdfs:domain rdf:resource="http://example.org/onto/class/yandex_mdb_clickhouse_cluster"/>
    <rdfs:range rdf:resource="http://www.w3.org/2001/XMLSchema#string"/>
  </owl:DatatypeProperty>
  <owl:DatatypeProperty rdf:about="http://example.org/onto/prop/yandex_mdb_clickhouse_cluster_max_memory_usage">
    <rdfs:label>max_memory_usage</rdfs:label>
    <rdfs:comment>Limits the maximum memory usage (in bytes) for processing queries on a single server.</rdfs:comment>
    <rdfs:domain rdf:resource="http://example.org/onto/class/yandex_mdb_clickhouse_cluster"/>
    <rdfs:range rdf:resource="http://www.w3.org/2001/XMLSchema#string"/>
  </owl:DatatypeProperty>
  <owl:DatatypeProperty rdf:about="http://example.org/onto/prop/yandex_mdb_clickhouse_cluster_max_memory_usage_for_user">
    <rdfs:label>max_memory_usage_for_user</rdfs:label>
    <rdfs:comment>Limits the maximum memory usage (in bytes) for processing of user's queries on a single server.</rdfs:comment>
    <rdfs:domain rdf:resource="http://example.org/onto/class/yandex_mdb_clickhouse_cluster"/>
    <rdfs:range rdf:resource="http://www.w3.org/2001/XMLSchema#string"/>
  </owl:DatatypeProperty>
  <owl:DatatypeProperty rdf:about="http://example.org/onto/prop/yandex_mdb_clickhouse_cluster_max_network_bandwidth">
    <rdfs:label>max_network_bandwidth</rdfs:label>
    <rdfs:comment>Limits the speed of the data exchange over the network in bytes per second.</rdfs:comment>
    <rdfs:domain rdf:resource="http://example.org/onto/class/yandex_mdb_clickhouse_cluster"/>
    <rdfs:range rdf:resource="http://www.w3.org/2001/XMLSchema#string"/>
  </owl:DatatypeProperty>
  <owl:DatatypeProperty rdf:about="http://example.org/onto/prop/yandex_mdb_clickhouse_cluster_max_network_bandwidth_for_user">
    <rdfs:label>max_network_bandwidth_for_user</rdfs:label>
    <rdfs:comment>Limits the speed of the data exchange over the network in bytes per second.</rdfs:comment>
    <rdfs:domain rdf:resource="http://example.org/onto/class/yandex_mdb_clickhouse_cluster"/>
    <rdfs:range rdf:resource="http://www.w3.org/2001/XMLSchema#string"/>
  </owl:DatatypeProperty>
  <owl:DatatypeProperty rdf:about="http://example.org/onto/prop/yandex_mdb_clickhouse_cluster_max_parser_depth">
    <rdfs:label>max_parser_depth</rdfs:label>
    <rdfs:comment>Limits maximum recursion depth in the recursive descent parser. Allows controlling the stack size. Zero means unlimited.</rdfs:comment>
    <rdfs:domain rdf:resource="http://example.org/onto/class/yandex_mdb_clickhouse_cluster"/>
    <rdfs:range rdf:resource="http://www.w3.org/2001/XMLSchema#string"/>
  </owl:DatatypeProperty>
  <owl:DatatypeProperty rdf:about="http://example.org/onto/prop/yandex_mdb_clickhouse_cluster_max_query_size">
    <rdfs:label>max_query_size</rdfs:label>
    <rdfs:comment>The maximum part of a query that can be taken to RAM for parsing with the SQL parser.</rdfs:comment>
    <rdfs:domain rdf:resource="http://example.org/onto/class/yandex_mdb_clickhouse_cluster"/>
    <rdfs:range rdf:resource="http://www.w3.org/2001/XMLSchema#string"/>
  </owl:DatatypeProperty>
  <owl:DatatypeProperty rdf:about="http://example.org/onto/prop/yandex_mdb_clickhouse_cluster_max_read_buffer_size">
    <rdfs:label>max_read_buffer_size</rdfs:label>
    <rdfs:comment>The maximum size of the buffer to read from the filesystem.</rdfs:comment>
    <rdfs:domain rdf:resource="http://example.org/onto/class/yandex_mdb_clickhouse_cluster"/>
    <rdfs:range rdf:resource="http://www.w3.org/2001/XMLSchema#string"/>
  </owl:DatatypeProperty>
  <owl:DatatypeProperty rdf:about="http://example.org/onto/prop/yandex_mdb_clickhouse_cluster_max_replica_delay_for_distributed_queries">
    <rdfs:label>max_replica_delay_for_distributed_queries</rdfs:label>
    <rdfs:comment>Disables lagging replicas for distributed queries.</rdfs:comment>
    <rdfs:domain rdf:resource="http://example.org/onto/class/yandex_mdb_clickhouse_cluster"/>
    <rdfs:range rdf:resource="http://www.w3.org/2001/XMLSchema#string"/>
  </owl:DatatypeProperty>
  <owl:DatatypeProperty rdf:about="http://example.org/onto/prop/yandex_mdb_clickhouse_cluster_max_result_bytes">
    <rdfs:label>max_result_bytes</rdfs:label>
    <rdfs:comment>Limits the number of bytes in the result.</rdfs:comment>
    <rdfs:domain rdf:resource="http://example.org/onto/class/yandex_mdb_clickhouse_cluster"/>
    <rdfs:range rdf:resource="http://www.w3.org/2001/XMLSchema#string"/>
  </owl:DatatypeProperty>
  <owl:DatatypeProperty rdf:about="http://example.org/onto/prop/yandex_mdb_clickhouse_cluster_max_result_rows">
    <rdfs:label>max_result_rows</rdfs:label>
    <rdfs:comment>Limits the number of rows in the result.</rdfs:comment>
    <rdfs:domain rdf:resource="http://example.org/onto/class/yandex_mdb_clickhouse_cluster"/>
    <rdfs:range rdf:resource="http://www.w3.org/2001/XMLSchema#string"/>
  </owl:DatatypeProperty>
  <owl:DatatypeProperty rdf:about="http://example.org/onto/prop/yandex_mdb_clickhouse_cluster_max_rows_in_distinct">
    <rdfs:label>max_rows_in_distinct</rdfs:label>
    <rdfs:comment>Limits the maximum number of different rows when using DISTINCT.</rdfs:comment>
    <rdfs:domain rdf:resource="http://example.org/onto/class/yandex_mdb_clickhouse_cluster"/>
    <rdfs:range rdf:resource="http://www.w3.org/2001/XMLSchema#string"/>
  </owl:DatatypeProperty>
  <owl:DatatypeProperty rdf:about="http://example.org/onto/prop/yandex_mdb_clickhouse_cluster_max_rows_in_join">
    <rdfs:label>max_rows_in_join</rdfs:label>
    <rdfs:comment>Limit on maximum size of the hash table for JOIN, in rows.</rdfs:comment>
    <rdfs:domain rdf:resource="http://example.org/onto/class/yandex_mdb_clickhouse_cluster"/>
    <rdfs:range rdf:resource="http://www.w3.org/2001/XMLSchema#string"/>
  </owl:DatatypeProperty>
  <owl:DatatypeProperty rdf:about="http://example.org/onto/prop/yandex_mdb_clickhouse_cluster_max_rows_in_set">
    <rdfs:label>max_rows_in_set</rdfs:label>
    <rdfs:comment>Limit on the number of rows in the set resulting from the execution of the IN section.</rdfs:comment>
    <rdfs:domain rdf:resource="http://example.org/onto/class/yandex_mdb_clickhouse_cluster"/>
    <rdfs:range rdf:resource="http://www.w3.org/2001/XMLSchema#string"/>
  </owl:DatatypeProperty>
  <owl:DatatypeProperty rdf:about="http://example.org/onto/prop/yandex_mdb_clickhouse_cluster_max_rows_to_group_by">
    <rdfs:label>max_rows_to_group_by</rdfs:label>
    <rdfs:comment>Limits the maximum number of unique keys received from aggregation function.</rdfs:comment>
    <rdfs:domain rdf:resource="http://example.org/onto/class/yandex_mdb_clickhouse_cluster"/>
    <rdfs:range rdf:resource="http://www.w3.org/2001/XMLSchema#string"/>
  </owl:DatatypeProperty>
  <owl:DatatypeProperty rdf:about="http://example.org/onto/prop/yandex_mdb_clickhouse_cluster_max_rows_to_read">
    <rdfs:label>max_rows_to_read</rdfs:label>
    <rdfs:comment>Limits the maximum number of rows that can be read from a table when running a query.</rdfs:comment>
    <rdfs:domain rdf:resource="http://example.org/onto/class/yandex_mdb_clickhouse_cluster"/>
    <rdfs:range rdf:resource="http://www.w3.org/2001/XMLSchema#string"/>
  </owl:DatatypeProperty>
  <owl:DatatypeProperty rdf:about="http://example.org/onto/prop/yandex_mdb_clickhouse_cluster_max_rows_to_sort">
    <rdfs:label>max_rows_to_sort</rdfs:label>
    <rdfs:comment>Limits the maximum number of rows that can be read from a table for sorting.</rdfs:comment>
    <rdfs:domain rdf:resource="http://example.org/onto/class/yandex_mdb_clickhouse_cluster"/>
    <rdfs:range rdf:resource="http://www.w3.org/2001/XMLSchema#string"/>
  </owl:DatatypeProperty>
  <owl:DatatypeProperty rdf:about="http://example.org/onto/prop/yandex_mdb_clickhouse_cluster_max_rows_to_transfer">
    <rdfs:label>max_rows_to_transfer</rdfs:label>
    <rdfs:comment>Limits the maximum number of rows that can be passed to a remote server or saved in a temporary table when using GLOBAL IN.</rdfs:comment>
    <rdfs:domain rdf:resource="http://example.org/onto/class/yandex_mdb_clickhouse_cluster"/>
    <rdfs:range rdf:resource="http://www.w3.org/2001/XMLSchema#string"/>
  </owl:DatatypeProperty>
  <owl:DatatypeProperty rdf:about="http://example.org/onto/prop/yandex_mdb_clickhouse_cluster_max_temporary_columns">
    <rdfs:label>max_temporary_columns</rdfs:label>
    <rdfs:comment>Limits the maximum number of temporary columns that must be kept in RAM at the same time when running a query, including constant columns.</rdfs:comment>
    <rdfs:domain rdf:resource="http://example.org/onto/class/yandex_mdb_clickhouse_cluster"/>
    <rdfs:range rdf:resource="http://www.w3.org/2001/XMLSchema#string"/>
  </owl:DatatypeProperty>
  <owl:DatatypeProperty rdf:about="http://example.org/onto/prop/yandex_mdb_clickhouse_cluster_max_temporary_data_on_disk_size_for_query">
    <rdfs:label>max_temporary_data_on_disk_size_for_query</rdfs:label>
    <rdfs:comment>The maximum amount of data consumed by temporary files on disk in bytes for all concurrently running queries. Zero means unlimited.</rdfs:comment>
    <rdfs:domain rdf:resource="http://example.org/onto/class/yandex_mdb_clickhouse_cluster"/>
    <rdfs:range rdf:resource="http://www.w3.org/2001/XMLSchema#string"/>
  </owl:DatatypeProperty>
  <owl:DatatypeProperty rdf:about="http://example.org/onto/prop/yandex_mdb_clickhouse_cluster_max_temporary_data_on_disk_size_for_user">
    <rdfs:label>max_temporary_data_on_disk_size_for_user</rdfs:label>
    <rdfs:comment>The maximum amount of data consumed by temporary files on disk in bytes for all concurrently running user queries. Zero means unlimited.</rdfs:comment>
    <rdfs:domain rdf:resource="http://example.org/onto/class/yandex_mdb_clickhouse_cluster"/>
    <rdfs:range rdf:resource="http://www.w3.org/2001/XMLSchema#string"/>
  </owl:DatatypeProperty>
  <owl:DatatypeProperty rdf:about="http://example.org/onto/prop/yandex_mdb_clickhouse_cluster_max_temporary_non_const_columns">
    <rdfs:label>max_temporary_non_const_columns</rdfs:label>
    <rdfs:comment>Limits the maximum number of temporary columns that must be kept in RAM at the same time when running a query, excluding constant columns.</rdfs:comment>
    <rdfs:domain rdf:resource="http://example.org/onto/class/yandex_mdb_clickhouse_cluster"/>
    <rdfs:range rdf:resource="http://www.w3.org/2001/XMLSchema#string"/>
  </owl:DatatypeProperty>
  <owl:DatatypeProperty rdf:about="http://example.org/onto/prop/yandex_mdb_clickhouse_cluster_max_threads">
    <rdfs:label>max_threads</rdfs:label>
    <rdfs:comment>The maximum number of query processing threads, excluding threads for retrieving data from remote servers.</rdfs:comment>
    <rdfs:domain rdf:resource="http://example.org/onto/class/yandex_mdb_clickhouse_cluster"/>
    <rdfs:range rdf:resource="http://www.w3.org/2001/XMLSchema#string"/>
  </owl:DatatypeProperty>
  <owl:DatatypeProperty rdf:about="http://example.org/onto/prop/yandex_mdb_clickhouse_cluster_memory_overcommit_ratio_denominator">
    <rdfs:label>memory_overcommit_ratio_denominator</rdfs:label>
    <rdfs:comment>It represents soft memory limit in case when hard limit is reached on user level. This value is used to compute overcommit ratio for the query. Zero means skip the query.</rdfs:comment>
    <rdfs:domain rdf:resource="http://example.org/onto/class/yandex_mdb_clickhouse_cluster"/>
    <rdfs:range rdf:resource="http://www.w3.org/2001/XMLSchema#string"/>
  </owl:DatatypeProperty>
  <owl:DatatypeProperty rdf:about="http://example.org/onto/prop/yandex_mdb_clickhouse_cluster_memory_overcommit_ratio_denominator_for_user">
    <rdfs:label>memory_overcommit_ratio_denominator_for_user</rdfs:label>
    <rdfs:comment>It represents soft memory limit in case when hard limit is reached on global level. This value is used to compute overcommit ratio for the query. Zero means skip the query.</rdfs:comment>
    <rdfs:domain rdf:resource="http://example.org/onto/class/yandex_mdb_clickhouse_cluster"/>
    <rdfs:range rdf:resource="http://www.w3.org/2001/XMLSchema#string"/>
  </owl:DatatypeProperty>
  <owl:DatatypeProperty rdf:about="http://example.org/onto/prop/yandex_mdb_clickhouse_cluster_memory_profiler_sample_probability">
    <rdfs:label>memory_profiler_sample_probability</rdfs:label>
    <rdfs:comment>Collect random allocations and deallocations and write them into system.trace_log with 'MemorySample' trace_type. The probability is for every alloc/free regardless to the size of the allocation. Possible values: from 0 to 1. Default: 0.</rdfs:comment>
    <rdfs:domain rdf:resource="http://example.org/onto/class/yandex_mdb_clickhouse_cluster"/>
    <rdfs:range rdf:resource="http://www.w3.org/2001/XMLSchema#string"/>
  </owl:DatatypeProperty>
  <owl:DatatypeProperty rdf:about="http://example.org/onto/prop/yandex_mdb_clickhouse_cluster_memory_profiler_step">
    <rdfs:label>memory_profiler_step</rdfs:label>
    <rdfs:comment>Memory profiler step (in bytes). If the next query step requires more memory than this parameter specifies, the memory profiler collects the allocating stack trace. Values lower than a few megabytes slow down query processing. Default value: 4194304 (4 MB). Zero means disabled memory profiler.</rdfs:comment>
    <rdfs:domain rdf:resource="http://example.org/onto/class/yandex_mdb_clickhouse_cluster"/>
    <rdfs:range rdf:resource="http://www.w3.org/2001/XMLSchema#string"/>
  </owl:DatatypeProperty>
  <owl:DatatypeProperty rdf:about="http://example.org/onto/prop/yandex_mdb_clickhouse_cluster_memory_usage_overcommit_max_wait_microseconds">
    <rdfs:label>memory_usage_overcommit_max_wait_microseconds</rdfs:label>
    <rdfs:comment>Maximum time thread will wait for memory to be freed in the case of memory overcommit on a user level. If the timeout is reached and memory is not freed, an exception is thrown.</rdfs:comment>
    <rdfs:domain rdf:resource="http://example.org/onto/class/yandex_mdb_clickhouse_cluster"/>
    <rdfs:range rdf:resource="http://www.w3.org/2001/XMLSchema#string"/>
  </owl:DatatypeProperty>
  <owl:DatatypeProperty rdf:about="http://example.org/onto/prop/yandex_mdb_clickhouse_cluster_merge_tree_max_bytes_to_use_cache">
    <rdfs:label>merge_tree_max_bytes_to_use_cache</rdfs:label>
    <rdfs:comment>If ClickHouse should read more than merge_tree_max_bytes_to_use_cache bytes in one query, it doesn’t use the cache of uncompressed blocks.</rdfs:comment>
    <rdfs:domain rdf:resource="http://example.org/onto/class/yandex_mdb_clickhouse_cluster"/>
    <rdfs:range rdf:resource="http://www.w3.org/2001/XMLSchema#string"/>
  </owl:DatatypeProperty>
  <owl:DatatypeProperty rdf:about="http://example.org/onto/prop/yandex_mdb_clickhouse_cluster_merge_tree_max_rows_to_use_cache">
    <rdfs:label>merge_tree_max_rows_to_use_cache</rdfs:label>
    <rdfs:comment>If ClickHouse should read more than merge_tree_max_rows_to_use_cache rows in one query, it doesn’t use the cache of uncompressed blocks.</rdfs:comment>
    <rdfs:domain rdf:resource="http://example.org/onto/class/yandex_mdb_clickhouse_cluster"/>
    <rdfs:range rdf:resource="http://www.w3.org/2001/XMLSchema#string"/>
  </owl:DatatypeProperty>
  <owl:DatatypeProperty rdf:about="http://example.org/onto/prop/yandex_mdb_clickhouse_cluster_merge_tree_min_bytes_for_concurrent_read">
    <rdfs:label>merge_tree_min_bytes_for_concurrent_read</rdfs:label>
    <rdfs:comment>If the number of bytes to read from one file of a MergeTree-engine table exceeds merge_tree_min_bytes_for_concurrent_read, then ClickHouse tries to concurrently read from this file in several threads.</rdfs:comment>
    <rdfs:domain rdf:resource="http://example.org/onto/class/yandex_mdb_clickhouse_cluster"/>
    <rdfs:range rdf:resource="http://www.w3.org/2001/XMLSchema#string"/>
  </owl:DatatypeProperty>
  <owl:DatatypeProperty rdf:about="http://example.org/onto/prop/yandex_mdb_clickhouse_cluster_merge_tree_min_rows_for_concurrent_read">
    <rdfs:label>merge_tree_min_rows_for_concurrent_read</rdfs:label>
    <rdfs:comment>If the number of rows to be read from a file of a MergeTree table exceeds merge_tree_min_rows_for_concurrent_read then ClickHouse tries to perform a concurrent reading from this file on several threads.</rdfs:comment>
    <rdfs:domain rdf:resource="http://example.org/onto/class/yandex_mdb_clickhouse_cluster"/>
    <rdfs:range rdf:resource="http://www.w3.org/2001/XMLSchema#string"/>
  </owl:DatatypeProperty>
  <owl:DatatypeProperty rdf:about="http://example.org/onto/prop/yandex_mdb_clickhouse_cluster_min_bytes_to_use_direct_io">
    <rdfs:label>min_bytes_to_use_direct_io</rdfs:label>
    <rdfs:comment>The minimum data volume required for using direct I/O access to the storage disk.</rdfs:comment>
    <rdfs:domain rdf:resource="http://example.org/onto/class/yandex_mdb_clickhouse_cluster"/>
    <rdfs:range rdf:resource="http://www.w3.org/2001/XMLSchema#string"/>
  </owl:DatatypeProperty>
  <owl:DatatypeProperty rdf:about="http://example.org/onto/prop/yandex_mdb_clickhouse_cluster_min_count_to_compile">
    <rdfs:label>min_count_to_compile</rdfs:label>
    <rdfs:comment>How many times to potentially use a compiled chunk of code before running compilation.</rdfs:comment>
    <rdfs:domain rdf:resource="http://example.org/onto/class/yandex_mdb_clickhouse_cluster"/>
    <rdfs:range rdf:resource="http://www.w3.org/2001/XMLSchema#string"/>
  </owl:DatatypeProperty>
  <owl:DatatypeProperty rdf:about="http://example.org/onto/prop/yandex_mdb_clickhouse_cluster_min_count_to_compile_expression">
    <rdfs:label>min_count_to_compile_expression</rdfs:label>
    <rdfs:comment>A query waits for expression compilation process to complete prior to continuing execution.</rdfs:comment>
    <rdfs:domain rdf:resource="http://example.org/onto/class/yandex_mdb_clickhouse_cluster"/>
    <rdfs:range rdf:resource="http://www.w3.org/2001/XMLSchema#string"/>
  </owl:DatatypeProperty>
  <owl:DatatypeProperty rdf:about="http://example.org/onto/prop/yandex_mdb_clickhouse_cluster_min_execution_speed">
    <rdfs:label>min_execution_speed</rdfs:label>
    <rdfs:comment>Minimal execution speed in rows per second.</rdfs:comment>
    <rdfs:domain rdf:resource="http://example.org/onto/class/yandex_mdb_clickhouse_cluster"/>
    <rdfs:range rdf:resource="http://www.w3.org/2001/XMLSchema#string"/>
  </owl:DatatypeProperty>
  <owl:DatatypeProperty rdf:about="http://example.org/onto/prop/yandex_mdb_clickhouse_cluster_min_execution_speed_bytes">
    <rdfs:label>min_execution_speed_bytes</rdfs:label>
    <rdfs:comment>Minimal execution speed in bytes per second.</rdfs:comment>
    <rdfs:domain rdf:resource="http://example.org/onto/class/yandex_mdb_clickhouse_cluster"/>
    <rdfs:range rdf:resource="http://www.w3.org/2001/XMLSchema#string"/>
  </owl:DatatypeProperty>
  <owl:DatatypeProperty rdf:about="http://example.org/onto/prop/yandex_mdb_clickhouse_cluster_min_insert_block_size_bytes">
    <rdfs:label>min_insert_block_size_bytes</rdfs:label>
    <rdfs:comment>Sets the minimum number of bytes in the block which can be inserted into a table by an INSERT query.</rdfs:comment>
    <rdfs:domain rdf:resource="http://example.org/onto/class/yandex_mdb_clickhouse_cluster"/>
    <rdfs:range rdf:resource="http://www.w3.org/2001/XMLSchema#string"/>
  </owl:DatatypeProperty>
  <owl:DatatypeProperty rdf:about="http://example.org/onto/prop/yandex_mdb_clickhouse_cluster_min_insert_block_size_rows">
    <rdfs:label>min_insert_block_size_rows</rdfs:label>
    <rdfs:comment>Sets the minimum number of rows in the block which can be inserted into a table by an INSERT query.</rdfs:comment>
    <rdfs:domain rdf:resource="http://example.org/onto/class/yandex_mdb_clickhouse_cluster"/>
    <rdfs:range rdf:resource="http://www.w3.org/2001/XMLSchema#string"/>
  </owl:DatatypeProperty>
  <owl:DatatypeProperty rdf:about="http://example.org/onto/prop/yandex_mdb_clickhouse_cluster_output_format_json_quote_64bit_integers">
    <rdfs:label>output_format_json_quote_64bit_integers</rdfs:label>
    <rdfs:comment>If the value is true, integers appear in quotes when using JSON* Int64 and UInt64 formats (for compatibility with most JavaScript implementations); otherwise, integers are output without the quotes.</rdfs:comment>
    <rdfs:domain rdf:resource="http://example.org/onto/class/yandex_mdb_clickhouse_cluster"/>
    <rdfs:range rdf:resource="http://www.w3.org/2001/XMLSchema#string"/>
  </owl:DatatypeProperty>
  <owl:DatatypeProperty rdf:about="http://example.org/onto/prop/yandex_mdb_clickhouse_cluster_output_format_json_quote_denormals">
    <rdfs:label>output_format_json_quote_denormals</rdfs:label>
    <rdfs:comment>Enables +nan, -nan, +inf, -inf outputs in JSON output format.</rdfs:comment>
    <rdfs:domain rdf:resource="http://example.org/onto/class/yandex_mdb_clickhouse_cluster"/>
    <rdfs:range rdf:resource="http://www.w3.org/2001/XMLSchema#string"/>
  </owl:DatatypeProperty>
  <owl:DatatypeProperty rdf:about="http://example.org/onto/prop/yandex_mdb_clickhouse_cluster_prefer_localhost_replica">
    <rdfs:label>prefer_localhost_replica</rdfs:label>
    <rdfs:comment>Enables/disables preferable using the localhost replica when processing distributed queries. Default value: true.</rdfs:comment>
    <rdfs:domain rdf:resource="http://example.org/onto/class/yandex_mdb_clickhouse_cluster"/>
    <rdfs:range rdf:resource="http://www.w3.org/2001/XMLSchema#string"/>
  </owl:DatatypeProperty>
  <owl:DatatypeProperty rdf:about="http://example.org/onto/prop/yandex_mdb_clickhouse_cluster_priority">
    <rdfs:label>priority</rdfs:label>
    <rdfs:comment>Query priority.</rdfs:comment>
    <rdfs:domain rdf:resource="http://example.org/onto/class/yandex_mdb_clickhouse_cluster"/>
    <rdfs:range rdf:resource="http://www.w3.org/2001/XMLSchema#string"/>
  </owl:DatatypeProperty>
  <owl:DatatypeProperty rdf:about="http://example.org/onto/prop/yandex_mdb_clickhouse_cluster_query_cache_max_entries">
    <rdfs:label>query_cache_max_entries</rdfs:label>
    <rdfs:comment>The maximum number of query results the current user may store in the query cache. 0 means unlimited.</rdfs:comment>
    <rdfs:domain rdf:resource="http://example.org/onto/class/yandex_mdb_clickhouse_cluster"/>
    <rdfs:range rdf:resource="http://www.w3.org/2001/XMLSchema#string"/>
  </owl:DatatypeProperty>
  <owl:DatatypeProperty rdf:about="http://example.org/onto/prop/yandex_mdb_clickhouse_cluster_query_cache_max_size_in_bytes">
    <rdfs:label>query_cache_max_size_in_bytes</rdfs:label>
    <rdfs:comment>The maximum amount of memory (in bytes) the current user may allocate in the query cache. 0 means unlimited.</rdfs:comment>
    <rdfs:domain rdf:resource="http://example.org/onto/class/yandex_mdb_clickhouse_cluster"/>
    <rdfs:range rdf:resource="http://www.w3.org/2001/XMLSchema#string"/>
  </owl:DatatypeProperty>
  <owl:DatatypeProperty rdf:about="http://example.org/onto/prop/yandex_mdb_clickhouse_cluster_query_cache_min_query_duration">
    <rdfs:label>query_cache_min_query_duration</rdfs:label>
    <rdfs:comment>Minimum duration in milliseconds a query needs to run for its result to be stored in the query cache.</rdfs:comment>
    <rdfs:domain rdf:resource="http://example.org/onto/class/yandex_mdb_clickhouse_cluster"/>
    <rdfs:range rdf:resource="http://www.w3.org/2001/XMLSchema#string"/>
  </owl:DatatypeProperty>
  <owl:DatatypeProperty rdf:about="http://example.org/onto/prop/yandex_mdb_clickhouse_cluster_query_cache_min_query_runs">
    <rdfs:label>query_cache_min_query_runs</rdfs:label>
    <rdfs:comment>Minimum number of times a SELECT query must run before its result is stored in the query cache.</rdfs:comment>
    <rdfs:domain rdf:resource="http://example.org/onto/class/yandex_mdb_clickhouse_cluster"/>
    <rdfs:range rdf:resource="http://www.w3.org/2001/XMLSchema#string"/>
  </owl:DatatypeProperty>
  <owl:DatatypeProperty rdf:about="http://example.org/onto/prop/yandex_mdb_clickhouse_cluster_query_cache_share_between_users">
    <rdfs:label>query_cache_share_between_users</rdfs:label>
    <rdfs:comment>If turned on, the result of SELECT queries cached in the query cache can be read by other users. It is not recommended to enable this setting due to security reasons.</rdfs:comment>
    <rdfs:domain rdf:resource="http://example.org/onto/class/yandex_mdb_clickhouse_cluster"/>
    <rdfs:range rdf:resource="http://www.w3.org/2001/XMLSchema#string"/>
  </owl:DatatypeProperty>
  <owl:DatatypeProperty rdf:about="http://example.org/onto/prop/yandex_mdb_clickhouse_cluster_query_cache_tag">
    <rdfs:label>query_cache_tag</rdfs:label>
    <rdfs:comment>A string which acts as a label for query cache entries. The same queries with different tags are considered different by the query cache.</rdfs:comment>
    <rdfs:domain rdf:resource="http://example.org/onto/class/yandex_mdb_clickhouse_cluster"/>
    <rdfs:range rdf:resource="http://www.w3.org/2001/XMLSchema#string"/>
  </owl:DatatypeProperty>
  <owl:DatatypeProperty rdf:about="http://example.org/onto/prop/yandex_mdb_clickhouse_cluster_query_cache_ttl">
    <rdfs:label>query_cache_ttl</rdfs:label>
    <rdfs:comment>After this time in seconds entries in the query cache become stale.</rdfs:comment>
    <rdfs:domain rdf:resource="http://example.org/onto/class/yandex_mdb_clickhouse_cluster"/>
    <rdfs:range rdf:resource="http://www.w3.org/2001/XMLSchema#string"/>
  </owl:DatatypeProperty>
  <owl:DatatypeProperty rdf:about="http://example.org/onto/prop/yandex_mdb_clickhouse_cluster_quota_mode">
    <rdfs:label>quota_mode</rdfs:label>
    <rdfs:comment>Quota accounting mode.</rdfs:comment>
    <rdfs:domain rdf:resource="http://example.org/onto/class/yandex_mdb_clickhouse_cluster"/>
    <rdfs:range rdf:resource="http://www.w3.org/2001/XMLSchema#string"/>
  </owl:DatatypeProperty>
  <owl:DatatypeProperty rdf:about="http://example.org/onto/prop/yandex_mdb_clickhouse_cluster_read_overflow_mode">
    <rdfs:label>read_overflow_mode</rdfs:label>
    <rdfs:comment>Sets behavior on overflow while read. Possible values:
* `throw` - abort query execution, return an error.
* `break` - stop query execution, return partial result.</rdfs:comment>
    <rdfs:domain rdf:resource="http://example.org/onto/class/yandex_mdb_clickhouse_cluster"/>
    <rdfs:range rdf:resource="http://www.w3.org/2001/XMLSchema#string"/>
  </owl:DatatypeProperty>
  <owl:DatatypeProperty rdf:about="http://example.org/onto/prop/yandex_mdb_clickhouse_cluster_readonly">
    <rdfs:label>readonly</rdfs:label>
    <rdfs:comment>Restricts permissions for reading data, write data and change settings queries.</rdfs:comment>
    <rdfs:domain rdf:resource="http://example.org/onto/class/yandex_mdb_clickhouse_cluster"/>
    <rdfs:range rdf:resource="http://www.w3.org/2001/XMLSchema#string"/>
  </owl:DatatypeProperty>
  <owl:DatatypeProperty rdf:about="http://example.org/onto/prop/yandex_mdb_clickhouse_cluster_receive_timeout">
    <rdfs:label>receive_timeout</rdfs:label>
    <rdfs:comment>Receive timeout in milliseconds on the socket used for communicating with the client.</rdfs:comment>
    <rdfs:domain rdf:resource="http://example.org/onto/class/yandex_mdb_clickhouse_cluster"/>
    <rdfs:range rdf:resource="http://www.w3.org/2001/XMLSchema#string"/>
  </owl:DatatypeProperty>
  <owl:DatatypeProperty rdf:about="http://example.org/onto/prop/yandex_mdb_clickhouse_cluster_remote_filesystem_read_method">
    <rdfs:label>remote_filesystem_read_method</rdfs:label>
    <rdfs:comment>Method of reading data from remote filesystem, one of: `read`, `threadpool`.</rdfs:comment>
    <rdfs:domain rdf:resource="http://example.org/onto/class/yandex_mdb_clickhouse_cluster"/>
    <rdfs:range rdf:resource="http://www.w3.org/2001/XMLSchema#string"/>
  </owl:DatatypeProperty>
  <owl:DatatypeProperty rdf:about="http://example.org/onto/prop/yandex_mdb_clickhouse_cluster_replication_alter_partitions_sync">
    <rdfs:label>replication_alter_partitions_sync</rdfs:label>
    <rdfs:comment>For ALTER ... ATTACH|DETACH|DROP queries, you can use the replication_alter_partitions_sync setting to set up waiting.</rdfs:comment>
    <rdfs:domain rdf:resource="http://example.org/onto/class/yandex_mdb_clickhouse_cluster"/>
    <rdfs:range rdf:resource="http://www.w3.org/2001/XMLSchema#string"/>
  </owl:DatatypeProperty>
  <owl:DatatypeProperty rdf:about="http://example.org/onto/prop/yandex_mdb_clickhouse_cluster_result_overflow_mode">
    <rdfs:label>result_overflow_mode</rdfs:label>
    <rdfs:comment>Sets behavior on overflow in result. Possible values:
* `throw` - abort query execution, return an error.
* `break` - stop query execution, return partial result.</rdfs:comment>
    <rdfs:domain rdf:resource="http://example.org/onto/class/yandex_mdb_clickhouse_cluster"/>
    <rdfs:range rdf:resource="http://www.w3.org/2001/XMLSchema#string"/>
  </owl:DatatypeProperty>
  <owl:DatatypeProperty rdf:about="http://example.org/onto/prop/yandex_mdb_clickhouse_cluster_s3_use_adaptive_timeouts">
    <rdfs:label>s3_use_adaptive_timeouts</rdfs:label>
    <rdfs:comment>Enables or disables adaptive timeouts for S3 requests.</rdfs:comment>
    <rdfs:domain rdf:resource="http://example.org/onto/class/yandex_mdb_clickhouse_cluster"/>
    <rdfs:range rdf:resource="http://www.w3.org/2001/XMLSchema#string"/>
  </owl:DatatypeProperty>
  <owl:DatatypeProperty rdf:about="http://example.org/onto/prop/yandex_mdb_clickhouse_cluster_select_sequential_consistency">
    <rdfs:label>select_sequential_consistency</rdfs:label>
    <rdfs:comment>Enables or disables sequential consistency for SELECT queries.</rdfs:comment>
    <rdfs:domain rdf:resource="http://example.org/onto/class/yandex_mdb_clickhouse_cluster"/>
    <rdfs:range rdf:resource="http://www.w3.org/2001/XMLSchema#string"/>
  </owl:DatatypeProperty>
  <owl:DatatypeProperty rdf:about="http://example.org/onto/prop/yandex_mdb_clickhouse_cluster_send_progress_in_http_headers">
    <rdfs:label>send_progress_in_http_headers</rdfs:label>
    <rdfs:comment>Enables or disables `X-ClickHouse-Progress` HTTP response headers in clickhouse-server responses.</rdfs:comment>
    <rdfs:domain rdf:resource="http://example.org/onto/class/yandex_mdb_clickhouse_cluster"/>
    <rdfs:range rdf:resource="http://www.w3.org/2001/XMLSchema#string"/>
  </owl:DatatypeProperty>
  <owl:DatatypeProperty rdf:about="http://example.org/onto/prop/yandex_mdb_clickhouse_cluster_send_timeout">
    <rdfs:label>send_timeout</rdfs:label>
    <rdfs:comment>Send timeout in milliseconds on the socket used for communicating with the client.</rdfs:comment>
    <rdfs:domain rdf:resource="http://example.org/onto/class/yandex_mdb_clickhouse_cluster"/>
    <rdfs:range rdf:resource="http://www.w3.org/2001/XMLSchema#string"/>
  </owl:DatatypeProperty>
  <owl:DatatypeProperty rdf:about="http://example.org/onto/prop/yandex_mdb_clickhouse_cluster_set_overflow_mode">
    <rdfs:label>set_overflow_mode</rdfs:label>
    <rdfs:comment>Sets behavior on overflow in the set resulting. Possible values:
  * `throw` - abort query execution, return an error.
* `break` - stop query execution, return partial result.</rdfs:comment>
    <rdfs:domain rdf:resource="http://example.org/onto/class/yandex_mdb_clickhouse_cluster"/>
    <rdfs:range rdf:resource="http://www.w3.org/2001/XMLSchema#string"/>
  </owl:DatatypeProperty>
  <owl:DatatypeProperty rdf:about="http://example.org/onto/prop/yandex_mdb_clickhouse_cluster_skip_unavailable_shards">
    <rdfs:label>skip_unavailable_shards</rdfs:label>
    <rdfs:comment>Enables or disables silently skipping of unavailable shards.</rdfs:comment>
    <rdfs:domain rdf:resource="http://example.org/onto/class/yandex_mdb_clickhouse_cluster"/>
    <rdfs:range rdf:resource="http://www.w3.org/2001/XMLSchema#string"/>
  </owl:DatatypeProperty>
  <owl:DatatypeProperty rdf:about="http://example.org/onto/prop/yandex_mdb_clickhouse_cluster_sort_overflow_mode">
    <rdfs:label>sort_overflow_mode</rdfs:label>
    <rdfs:comment>Sets behavior on overflow while sort. Possible values:
* `throw` - abort query execution, return an error.
* `break` - stop query execution, return partial result.</rdfs:comment>
    <rdfs:domain rdf:resource="http://example.org/onto/class/yandex_mdb_clickhouse_cluster"/>
    <rdfs:range rdf:resource="http://www.w3.org/2001/XMLSchema#string"/>
  </owl:DatatypeProperty>
  <owl:DatatypeProperty rdf:about="http://example.org/onto/prop/yandex_mdb_clickhouse_cluster_timeout_before_checking_execution_speed">
    <rdfs:label>timeout_before_checking_execution_speed</rdfs:label>
    <rdfs:comment>Timeout (in seconds) between checks of execution speed. It is checked that execution speed is not less that specified in min_execution_speed parameter. Must be at least 1000.</rdfs:comment>
    <rdfs:domain rdf:resource="http://example.org/onto/class/yandex_mdb_clickhouse_cluster"/>
    <rdfs:range rdf:resource="http://www.w3.org/2001/XMLSchema#string"/>
  </owl:DatatypeProperty>
  <owl:DatatypeProperty rdf:about="http://example.org/onto/prop/yandex_mdb_clickhouse_cluster_timeout_overflow_mode">
    <rdfs:label>timeout_overflow_mode</rdfs:label>
    <rdfs:comment>Sets behavior on overflow. Possible values:
* `throw` - abort query execution, return an error.
* `break` - stop query execution, return partial result.</rdfs:comment>
    <rdfs:domain rdf:resource="http://example.org/onto/class/yandex_mdb_clickhouse_cluster"/>
    <rdfs:range rdf:resource="http://www.w3.org/2001/XMLSchema#string"/>
  </owl:DatatypeProperty>
  <owl:DatatypeProperty rdf:about="http://example.org/onto/prop/yandex_mdb_clickhouse_cluster_transfer_overflow_mode">
    <rdfs:label>transfer_overflow_mode</rdfs:label>
    <rdfs:comment>Sets behavior on overflow. Possible values:
* `throw` - abort query execution, return an error.
* `break` - stop query execution, return partial result.</rdfs:comment>
    <rdfs:domain rdf:resource="http://example.org/onto/class/yandex_mdb_clickhouse_cluster"/>
    <rdfs:range rdf:resource="http://www.w3.org/2001/XMLSchema#string"/>
  </owl:DatatypeProperty>
  <owl:DatatypeProperty rdf:about="http://example.org/onto/prop/yandex_mdb_clickhouse_cluster_transform_null_in">
    <rdfs:label>transform_null_in</rdfs:label>
    <rdfs:comment>Enables equality of NULL values for IN operator.</rdfs:comment>
    <rdfs:domain rdf:resource="http://example.org/onto/class/yandex_mdb_clickhouse_cluster"/>
    <rdfs:range rdf:resource="http://www.w3.org/2001/XMLSchema#string"/>
  </owl:DatatypeProperty>
  <owl:DatatypeProperty rdf:about="http://example.org/onto/prop/yandex_mdb_clickhouse_cluster_use_hedged_requests">
    <rdfs:label>use_hedged_requests</rdfs:label>
    <rdfs:comment>Enables hedged requests logic for remote queries. It allows to establish many connections with different replicas for query. New connection is enabled in case existent connection(s) with replica(s) were not established within hedged_connection_timeout or no data was received within receive_data_timeout. Query uses the first connection which send non empty progress packet (or data packet, if allow_changing_replica_until_first_data_packet); other connections are cancelled. Queries with max_parallel_replicas > 1 are supported. Default value: true.</rdfs:comment>
    <rdfs:domain rdf:resource="http://example.org/onto/class/yandex_mdb_clickhouse_cluster"/>
    <rdfs:range rdf:resource="http://www.w3.org/2001/XMLSchema#string"/>
  </owl:DatatypeProperty>
  <owl:DatatypeProperty rdf:about="http://example.org/onto/prop/yandex_mdb_clickhouse_cluster_use_query_cache">
    <rdfs:label>use_query_cache</rdfs:label>
    <rdfs:comment>If turned on, SELECT queries may utilize the query cache.</rdfs:comment>
    <rdfs:domain rdf:resource="http://example.org/onto/class/yandex_mdb_clickhouse_cluster"/>
    <rdfs:range rdf:resource="http://www.w3.org/2001/XMLSchema#string"/>
  </owl:DatatypeProperty>
  <owl:DatatypeProperty rdf:about="http://example.org/onto/prop/yandex_mdb_clickhouse_cluster_use_uncompressed_cache">
    <rdfs:label>use_uncompressed_cache</rdfs:label>
    <rdfs:comment>Whether to use a cache of uncompressed blocks.</rdfs:comment>
    <rdfs:domain rdf:resource="http://example.org/onto/class/yandex_mdb_clickhouse_cluster"/>
    <rdfs:range rdf:resource="http://www.w3.org/2001/XMLSchema#string"/>
  </owl:DatatypeProperty>
  <owl:DatatypeProperty rdf:about="http://example.org/onto/prop/yandex_mdb_clickhouse_cluster_wait_for_async_insert">
    <rdfs:label>wait_for_async_insert</rdfs:label>
    <rdfs:comment>Enables waiting for processing of asynchronous insertion. If enabled, server returns OK only after the data is inserted.</rdfs:comment>
    <rdfs:domain rdf:resource="http://example.org/onto/class/yandex_mdb_clickhouse_cluster"/>
    <rdfs:range rdf:resource="http://www.w3.org/2001/XMLSchema#string"/>
  </owl:DatatypeProperty>
  <owl:DatatypeProperty rdf:about="http://example.org/onto/prop/yandex_mdb_clickhouse_cluster_wait_for_async_insert_timeout">
    <rdfs:label>wait_for_async_insert_timeout</rdfs:label>
    <rdfs:comment>The timeout (in seconds) for waiting for processing of asynchronous insertion. Value must be at least 1000 (1 second).</rdfs:comment>
    <rdfs:domain rdf:resource="http://example.org/onto/class/yandex_mdb_clickhouse_cluster"/>
    <rdfs:range rdf:resource="http://www.w3.org/2001/XMLSchema#string"/>
  </owl:DatatypeProperty>
  <owl:DatatypeProperty rdf:about="http://example.org/onto/prop/yandex_mdb_clickhouse_cluster_disk_size">
    <rdfs:label>disk_size</rdfs:label>
    <rdfs:comment>Volume of the storage available to a ZooKeeper host, in gigabytes.</rdfs:comment>
    <rdfs:domain rdf:resource="http://example.org/onto/class/yandex_mdb_clickhouse_cluster"/>
    <rdfs:range rdf:resource="http://www.w3.org/2001/XMLSchema#string"/>
  </owl:DatatypeProperty>
  <owl:DatatypeProperty rdf:about="http://example.org/onto/prop/yandex_mdb_clickhouse_cluster_disk_type_id">
    <rdfs:label>disk_type_id</rdfs:label>
    <rdfs:comment>Type of the storage of ZooKeeper hosts. For more information see [the official documentation](https://yandex.cloud/docs/managed-clickhouse/concepts/storage).</rdfs:comment>
    <rdfs:domain rdf:resource="http://example.org/onto/class/yandex_mdb_clickhouse_cluster"/>
    <rdfs:range rdf:resource="http://www.w3.org/2001/XMLSchema#string"/>
  </owl:DatatypeProperty>
  <owl:DatatypeProperty rdf:about="http://example.org/onto/prop/yandex_mdb_clickhouse_cluster_resource_preset_id">
    <rdfs:label>resource_preset_id</rdfs:label>
    <rdfs:comment>The ID of the preset for computational resources available to a ZooKeeper host (CPU, memory etc.). For more information, see [the official documentation](https://yandex.cloud/docs/managed-clickhouse/concepts).</rdfs:comment>
    <rdfs:domain rdf:resource="http://example.org/onto/class/yandex_mdb_clickhouse_cluster"/>
    <rdfs:range rdf:resource="http://www.w3.org/2001/XMLSchema#string"/>
  </owl:DatatypeProperty>
</rdf:RDF>
