<?xml version="1.0" encoding="UTF-8"?>
<rdf:RDF
  xmlns:rdf="http://www.w3.org/1999/02/22-rdf-syntax-ns#"
  xmlns:rdfs="http://www.w3.org/2000/01/rdf-schema#"
  xmlns:owl="http://www.w3.org/2002/07/owl#"
  xmlns:xsd="http://www.w3.org/2001/XMLSchema#"
  xml:base="http://example.org/onto/">
  <owl:Class rdf:about="http://example.org/onto/class/yandex_airflow_cluster">
    <rdfs:label>yandex_airflow_cluster</rdfs:label>
    <rdfs:comment>Managed Airflow cluster.</rdfs:comment>
  </owl:Class>
  <owl:DatatypeProperty rdf:about="http://example.org/onto/prop/yandex_airflow_cluster_admin_password">
    <rdfs:label>admin_password</rdfs:label>
    <rdfs:comment>Password that is used to log in to Apache Airflow web UI under `admin` user.</rdfs:comment>
    <rdfs:domain rdf:resource="http://example.org/onto/class/yandex_airflow_cluster"/>
    <rdfs:range rdf:resource="http://www.w3.org/2001/XMLSchema#string"/>
  </owl:DatatypeProperty>
  <owl:DatatypeProperty rdf:about="http://example.org/onto/prop/yandex_airflow_cluster_airflow_config">
    <rdfs:label>airflow_config</rdfs:label>
    <rdfs:comment>Configuration of the Apache Airflow application itself. The value of this attribute is a two-level map. Keys of top-level map are the names of [configuration sections](https://airflow.apache.org/docs/apache-airflow/stable/configurations-ref.html#airflow-configuration-options). Keys of inner maps are the names of configuration options within corresponding section.</rdfs:comment>
    <rdfs:domain rdf:resource="http://example.org/onto/class/yandex_airflow_cluster"/>
    <rdfs:range rdf:resource="http://www.w3.org/2001/XMLSchema#string"/>
  </owl:DatatypeProperty>
  <owl:DatatypeProperty rdf:about="http://example.org/onto/prop/yandex_airflow_cluster_airflow_version">
    <rdfs:label>airflow_version</rdfs:label>
    <rdfs:comment>Apache Airflow version in format `<major>.<minor>`.</rdfs:comment>
    <rdfs:domain rdf:resource="http://example.org/onto/class/yandex_airflow_cluster"/>
    <rdfs:range rdf:resource="http://www.w3.org/2001/XMLSchema#string"/>
  </owl:DatatypeProperty>
  <owl:DatatypeProperty rdf:about="http://example.org/onto/prop/yandex_airflow_cluster_code_sync">
    <rdfs:label>code_sync</rdfs:label>
    <rdfs:comment>Parameters of the location and access to the code that will be executed in the cluster.</rdfs:comment>
    <rdfs:domain rdf:resource="http://example.org/onto/class/yandex_airflow_cluster"/>
    <rdfs:range rdf:resource="http://www.w3.org/2001/XMLSchema#string"/>
  </owl:DatatypeProperty>
  <owl:DatatypeProperty rdf:about="http://example.org/onto/prop/yandex_airflow_cluster_created_at">
    <rdfs:label>created_at</rdfs:label>
    <rdfs:comment>The creation timestamp of the resource.</rdfs:comment>
    <rdfs:domain rdf:resource="http://example.org/onto/class/yandex_airflow_cluster"/>
    <rdfs:range rdf:resource="http://www.w3.org/2001/XMLSchema#string"/>
  </owl:DatatypeProperty>
  <owl:DatatypeProperty rdf:about="http://example.org/onto/prop/yandex_airflow_cluster_deb_packages">
    <rdfs:label>deb_packages</rdfs:label>
    <rdfs:comment>System packages that are installed in the cluster.</rdfs:comment>
    <rdfs:domain rdf:resource="http://example.org/onto/class/yandex_airflow_cluster"/>
    <rdfs:range rdf:resource="http://www.w3.org/2001/XMLSchema#string"/>
  </owl:DatatypeProperty>
  <owl:DatatypeProperty rdf:about="http://example.org/onto/prop/yandex_airflow_cluster_deletion_protection">
    <rdfs:label>deletion_protection</rdfs:label>
    <rdfs:comment>The `true` value means that resource is protected from accidental deletion.</rdfs:comment>
    <rdfs:domain rdf:resource="http://example.org/onto/class/yandex_airflow_cluster"/>
    <rdfs:range rdf:resource="http://www.w3.org/2001/XMLSchema#string"/>
  </owl:DatatypeProperty>
  <owl:DatatypeProperty rdf:about="http://example.org/onto/prop/yandex_airflow_cluster_description">
    <rdfs:label>description</rdfs:label>
    <rdfs:comment>The resource description.</rdfs:comment>
    <rdfs:domain rdf:resource="http://example.org/onto/class/yandex_airflow_cluster"/>
    <rdfs:range rdf:resource="http://www.w3.org/2001/XMLSchema#string"/>
  </owl:DatatypeProperty>
  <owl:DatatypeProperty rdf:about="http://example.org/onto/prop/yandex_airflow_cluster_folder_id">
    <rdfs:label>folder_id</rdfs:label>
    <rdfs:comment>The folder identifier that resource belongs to. If it is not provided, the default provider `folder-id` is used.</rdfs:comment>
    <rdfs:domain rdf:resource="http://example.org/onto/class/yandex_airflow_cluster"/>
    <rdfs:range rdf:resource="http://www.w3.org/2001/XMLSchema#string"/>
  </owl:DatatypeProperty>
  <owl:DatatypeProperty rdf:about="http://example.org/onto/prop/yandex_airflow_cluster_health">
    <rdfs:label>health</rdfs:label>
    <rdfs:comment>Aggregated health of the cluster. Can be either `ALIVE`, `DEGRADED`, `DEAD` or `HEALTH_UNKNOWN`. For more information see `health` field of JSON representation in [the official documentation](https://yandex.cloud/docs/managed-airflow/api-ref/Cluster/).</rdfs:comment>
    <rdfs:domain rdf:resource="http://example.org/onto/class/yandex_airflow_cluster"/>
    <rdfs:range rdf:resource="http://www.w3.org/2001/XMLSchema#string"/>
  </owl:DatatypeProperty>
  <owl:DatatypeProperty rdf:about="http://example.org/onto/prop/yandex_airflow_cluster_id">
    <rdfs:label>id</rdfs:label>
    <rdfs:comment>The resource identifier.</rdfs:comment>
    <rdfs:domain rdf:resource="http://example.org/onto/class/yandex_airflow_cluster"/>
    <rdfs:range rdf:resource="http://www.w3.org/2001/XMLSchema#string"/>
  </owl:DatatypeProperty>
  <owl:DatatypeProperty rdf:about="http://example.org/onto/prop/yandex_airflow_cluster_labels">
    <rdfs:label>labels</rdfs:label>
    <rdfs:comment>A set of key/value label pairs which assigned to resource.</rdfs:comment>
    <rdfs:domain rdf:resource="http://example.org/onto/class/yandex_airflow_cluster"/>
    <rdfs:range rdf:resource="http://www.w3.org/2001/XMLSchema#string"/>
  </owl:DatatypeProperty>
  <owl:DatatypeProperty rdf:about="http://example.org/onto/prop/yandex_airflow_cluster_lockbox_secrets_backend">
    <rdfs:label>lockbox_secrets_backend</rdfs:label>
    <rdfs:comment>Configuration of Lockbox Secrets Backend. [See documentation](https://yandex.cloud/docs/managed-airflow/tutorials/lockbox-secrets-in-maf-cluster) for details.</rdfs:comment>
    <rdfs:domain rdf:resource="http://example.org/onto/class/yandex_airflow_cluster"/>
    <rdfs:range rdf:resource="http://www.w3.org/2001/XMLSchema#string"/>
  </owl:DatatypeProperty>
  <owl:DatatypeProperty rdf:about="http://example.org/onto/prop/yandex_airflow_cluster_logging">
    <rdfs:label>logging</rdfs:label>
    <rdfs:comment>Cloud Logging configuration.</rdfs:comment>
    <rdfs:domain rdf:resource="http://example.org/onto/class/yandex_airflow_cluster"/>
    <rdfs:range rdf:resource="http://www.w3.org/2001/XMLSchema#string"/>
  </owl:DatatypeProperty>
  <owl:DatatypeProperty rdf:about="http://example.org/onto/prop/yandex_airflow_cluster_maintenance_window">
    <rdfs:label>maintenance_window</rdfs:label>
    <rdfs:comment>Configuration of window for maintenance operations.</rdfs:comment>
    <rdfs:domain rdf:resource="http://example.org/onto/class/yandex_airflow_cluster"/>
    <rdfs:range rdf:resource="http://www.w3.org/2001/XMLSchema#string"/>
  </owl:DatatypeProperty>
  <owl:DatatypeProperty rdf:about="http://example.org/onto/prop/yandex_airflow_cluster_name">
    <rdfs:label>name</rdfs:label>
    <rdfs:comment>The resource name.</rdfs:comment>
    <rdfs:domain rdf:resource="http://example.org/onto/class/yandex_airflow_cluster"/>
    <rdfs:range rdf:resource="http://www.w3.org/2001/XMLSchema#string"/>
  </owl:DatatypeProperty>
  <owl:DatatypeProperty rdf:about="http://example.org/onto/prop/yandex_airflow_cluster_pip_packages">
    <rdfs:label>pip_packages</rdfs:label>
    <rdfs:comment>Python packages that are installed in the cluster.</rdfs:comment>
    <rdfs:domain rdf:resource="http://example.org/onto/class/yandex_airflow_cluster"/>
    <rdfs:range rdf:resource="http://www.w3.org/2001/XMLSchema#string"/>
  </owl:DatatypeProperty>
  <owl:DatatypeProperty rdf:about="http://example.org/onto/prop/yandex_airflow_cluster_python_version">
    <rdfs:label>python_version</rdfs:label>
    <rdfs:comment>Version of Python that Airflow will run on. Must be in format `<major>.<minor>`.</rdfs:comment>
    <rdfs:domain rdf:resource="http://example.org/onto/class/yandex_airflow_cluster"/>
    <rdfs:range rdf:resource="http://www.w3.org/2001/XMLSchema#string"/>
  </owl:DatatypeProperty>
  <owl:DatatypeProperty rdf:about="http://example.org/onto/prop/yandex_airflow_cluster_scheduler">
    <rdfs:label>scheduler</rdfs:label>
    <rdfs:comment>Configuration of scheduler instances.</rdfs:comment>
    <rdfs:domain rdf:resource="http://example.org/onto/class/yandex_airflow_cluster"/>
    <rdfs:range rdf:resource="http://www.w3.org/2001/XMLSchema#string"/>
  </owl:DatatypeProperty>
  <owl:DatatypeProperty rdf:about="http://example.org/onto/prop/yandex_airflow_cluster_security_group_ids">
    <rdfs:label>security_group_ids</rdfs:label>
    <rdfs:comment>The list of security groups applied to resource or their components.</rdfs:comment>
    <rdfs:domain rdf:resource="http://example.org/onto/class/yandex_airflow_cluster"/>
    <rdfs:range rdf:resource="http://www.w3.org/2001/XMLSchema#string"/>
  </owl:DatatypeProperty>
  <owl:DatatypeProperty rdf:about="http://example.org/onto/prop/yandex_airflow_cluster_service_account_id">
    <rdfs:label>service_account_id</rdfs:label>
    <rdfs:comment>[Service account](https://yandex.cloud/docs/iam/concepts/users/service-accounts) which linked to the resource. For more information, see [documentation](https://yandex.cloud/docs/managed-airflow/concepts/impersonation).</rdfs:comment>
    <rdfs:domain rdf:resource="http://example.org/onto/class/yandex_airflow_cluster"/>
    <rdfs:range rdf:resource="http://www.w3.org/2001/XMLSchema#string"/>
  </owl:DatatypeProperty>
  <owl:DatatypeProperty rdf:about="http://example.org/onto/prop/yandex_airflow_cluster_status">
    <rdfs:label>status</rdfs:label>
    <rdfs:comment>Status of the cluster. Can be either `CREATING`, `STARTING`, `RUNNING`, `UPDATING`, `STOPPING`, `STOPPED`, `ERROR` or `STATUS_UNKNOWN`. For more information see `status` field of JSON representation in [the official documentation](https://yandex.cloud/docs/managed-airflow/api-ref/Cluster/).</rdfs:comment>
    <rdfs:domain rdf:resource="http://example.org/onto/class/yandex_airflow_cluster"/>
    <rdfs:range rdf:resource="http://www.w3.org/2001/XMLSchema#string"/>
  </owl:DatatypeProperty>
  <owl:DatatypeProperty rdf:about="http://example.org/onto/prop/yandex_airflow_cluster_subnet_ids">
    <rdfs:label>subnet_ids</rdfs:label>
    <rdfs:comment>The list of VPC subnets identifiers which resource is attached.</rdfs:comment>
    <rdfs:domain rdf:resource="http://example.org/onto/class/yandex_airflow_cluster"/>
    <rdfs:range rdf:resource="http://www.w3.org/2001/XMLSchema#string"/>
  </owl:DatatypeProperty>
  <owl:DatatypeProperty rdf:about="http://example.org/onto/prop/yandex_airflow_cluster_triggerer">
    <rdfs:label>triggerer</rdfs:label>
    <rdfs:comment>Configuration of `triggerer` instances.</rdfs:comment>
    <rdfs:domain rdf:resource="http://example.org/onto/class/yandex_airflow_cluster"/>
    <rdfs:range rdf:resource="http://www.w3.org/2001/XMLSchema#string"/>
  </owl:DatatypeProperty>
  <owl:DatatypeProperty rdf:about="http://example.org/onto/prop/yandex_airflow_cluster_webserver">
    <rdfs:label>webserver</rdfs:label>
    <rdfs:comment>Configuration of `webserver` instances.</rdfs:comment>
    <rdfs:domain rdf:resource="http://example.org/onto/class/yandex_airflow_cluster"/>
    <rdfs:range rdf:resource="http://www.w3.org/2001/XMLSchema#string"/>
  </owl:DatatypeProperty>
  <owl:DatatypeProperty rdf:about="http://example.org/onto/prop/yandex_airflow_cluster_worker">
    <rdfs:label>worker</rdfs:label>
    <rdfs:comment>Configuration of worker instances.</rdfs:comment>
    <rdfs:domain rdf:resource="http://example.org/onto/class/yandex_airflow_cluster"/>
    <rdfs:range rdf:resource="http://www.w3.org/2001/XMLSchema#string"/>
  </owl:DatatypeProperty>
  <owl:DatatypeProperty rdf:about="http://example.org/onto/prop/yandex_airflow_cluster_create">
    <rdfs:label>create</rdfs:label>
    <rdfs:comment>A string that can be [parsed as a duration](https://pkg.go.dev/time#ParseDuration) consisting of numbers and unit suffixes, such as "30s" or "2h45m". Valid time units are "s" (seconds), "m" (minutes), "h" (hours).</rdfs:comment>
    <rdfs:domain rdf:resource="http://example.org/onto/class/yandex_airflow_cluster"/>
    <rdfs:range rdf:resource="http://www.w3.org/2001/XMLSchema#string"/>
  </owl:DatatypeProperty>
  <owl:DatatypeProperty rdf:about="http://example.org/onto/prop/yandex_airflow_cluster_delete">
    <rdfs:label>delete</rdfs:label>
    <rdfs:comment>A string that can be [parsed as a duration](https://pkg.go.dev/time#ParseDuration) consisting of numbers and unit suffixes, such as "30s" or "2h45m". Valid time units are "s" (seconds), "m" (minutes), "h" (hours). Setting a timeout for a Delete operation is only applicable if changes are saved into state before the destroy operation occurs.</rdfs:comment>
    <rdfs:domain rdf:resource="http://example.org/onto/class/yandex_airflow_cluster"/>
    <rdfs:range rdf:resource="http://www.w3.org/2001/XMLSchema#string"/>
  </owl:DatatypeProperty>
  <owl:DatatypeProperty rdf:about="http://example.org/onto/prop/yandex_airflow_cluster_update">
    <rdfs:label>update</rdfs:label>
    <rdfs:comment>A string that can be [parsed as a duration](https://pkg.go.dev/time#ParseDuration) consisting of numbers and unit suffixes, such as "30s" or "2h45m". Valid time units are "s" (seconds), "m" (minutes), "h" (hours).</rdfs:comment>
    <rdfs:domain rdf:resource="http://example.org/onto/class/yandex_airflow_cluster"/>
    <rdfs:range rdf:resource="http://www.w3.org/2001/XMLSchema#string"/>
  </owl:DatatypeProperty>
</rdf:RDF>
