<?xml version="1.0" encoding="UTF-8"?>
<rdf:RDF
  xmlns:rdf="http://www.w3.org/1999/02/22-rdf-syntax-ns#"
  xmlns:rdfs="http://www.w3.org/2000/01/rdf-schema#"
  xmlns:owl="http://www.w3.org/2002/07/owl#"
  xmlns:xsd="http://www.w3.org/2001/XMLSchema#"
  xml:base="http://example.org/onto/">
  <owl:Class rdf:about="http://example.org/onto/class/yandex_iam_service_account">
    <rdfs:label>yandex_iam_service_account</rdfs:label>
    <rdfs:comment>A ServiceAccount resource. For more information, see [Service accounts](/docs/iam/concepts/users/service-accounts).</rdfs:comment>
  </owl:Class>
  <owl:DatatypeProperty rdf:about="http://example.org/onto/prop/yandex_iam_service_account_created_at">
    <rdfs:label>created_at</rdfs:label>
    <rdfs:comment>Creation timestamp.</rdfs:comment>
    <rdfs:domain rdf:resource="http://example.org/onto/class/yandex_iam_service_account"/>
    <rdfs:range rdf:resource="http://www.w3.org/2001/XMLSchema#string"/>
  </owl:DatatypeProperty>
  <owl:DatatypeProperty rdf:about="http://example.org/onto/prop/yandex_iam_service_account_description">
    <rdfs:label>description</rdfs:label>
    <rdfs:comment>Description of the service account. 0-256 characters long.</rdfs:comment>
    <rdfs:domain rdf:resource="http://example.org/onto/class/yandex_iam_service_account"/>
    <rdfs:range rdf:resource="http://www.w3.org/2001/XMLSchema#string"/>
  </owl:DatatypeProperty>
  <owl:DatatypeProperty rdf:about="http://example.org/onto/prop/yandex_iam_service_account_folder_id">
    <rdfs:label>folder_id</rdfs:label>
    <rdfs:comment>ID of the folder that the service account belongs to.</rdfs:comment>
    <rdfs:domain rdf:resource="http://example.org/onto/class/yandex_iam_service_account"/>
    <rdfs:range rdf:resource="http://www.w3.org/2001/XMLSchema#string"/>
  </owl:DatatypeProperty>
  <owl:DatatypeProperty rdf:about="http://example.org/onto/prop/yandex_iam_service_account_id">
    <rdfs:label>id</rdfs:label>
    <rdfs:comment>ID of the ServiceAccount resource to return.
 To get the service account ID, use a [ServiceAccountService.List] request.</rdfs:comment>
    <rdfs:domain rdf:resource="http://example.org/onto/class/yandex_iam_service_account"/>
    <rdfs:range rdf:resource="http://www.w3.org/2001/XMLSchema#string"/>
  </owl:DatatypeProperty>
  <owl:DatatypeProperty rdf:about="http://example.org/onto/prop/yandex_iam_service_account_name">
    <rdfs:label>name</rdfs:label>
    <rdfs:comment>Name of the service account.
 The name is unique within the cloud. 3-63 characters long.</rdfs:comment>
    <rdfs:domain rdf:resource="http://example.org/onto/class/yandex_iam_service_account"/>
    <rdfs:range rdf:resource="http://www.w3.org/2001/XMLSchema#string"/>
  </owl:DatatypeProperty>
  <owl:DatatypeProperty rdf:about="http://example.org/onto/prop/yandex_iam_service_account_service_account_id">
    <rdfs:label>service_account_id</rdfs:label>
    <rdfs:comment>ID of the ServiceAccount resource to return.
 To get the service account ID, use a [ServiceAccountService.List] request.</rdfs:comment>
    <rdfs:domain rdf:resource="http://example.org/onto/class/yandex_iam_service_account"/>
    <rdfs:range rdf:resource="http://www.w3.org/2001/XMLSchema#string"/>
  </owl:DatatypeProperty>
  <owl:DatatypeProperty rdf:about="http://example.org/onto/prop/yandex_iam_service_account_create">
    <rdfs:label>create</rdfs:label>
    <rdfs:comment>A string that can be [parsed as a duration](https://pkg.go.dev/time#ParseDuration) consisting of numbers and unit suffixes, such as "30s" or "2h45m". Valid time units are "s" (seconds), "m" (minutes), "h" (hours).</rdfs:comment>
    <rdfs:domain rdf:resource="http://example.org/onto/class/yandex_iam_service_account"/>
    <rdfs:range rdf:resource="http://www.w3.org/2001/XMLSchema#string"/>
  </owl:DatatypeProperty>
  <owl:DatatypeProperty rdf:about="http://example.org/onto/prop/yandex_iam_service_account_delete">
    <rdfs:label>delete</rdfs:label>
    <rdfs:comment>A string that can be [parsed as a duration](https://pkg.go.dev/time#ParseDuration) consisting of numbers and unit suffixes, such as "30s" or "2h45m". Valid time units are "s" (seconds), "m" (minutes), "h" (hours). Setting a timeout for a Delete operation is only applicable if changes are saved into state before the destroy operation occurs.</rdfs:comment>
    <rdfs:domain rdf:resource="http://example.org/onto/class/yandex_iam_service_account"/>
    <rdfs:range rdf:resource="http://www.w3.org/2001/XMLSchema#string"/>
  </owl:DatatypeProperty>
  <owl:DatatypeProperty rdf:about="http://example.org/onto/prop/yandex_iam_service_account_read">
    <rdfs:label>read</rdfs:label>
    <rdfs:comment>A string that can be [parsed as a duration](https://pkg.go.dev/time#ParseDuration) consisting of numbers and unit suffixes, such as "30s" or "2h45m". Valid time units are "s" (seconds), "m" (minutes), "h" (hours). Read operations occur during any refresh or planning operation when refresh is enabled.</rdfs:comment>
    <rdfs:domain rdf:resource="http://example.org/onto/class/yandex_iam_service_account"/>
    <rdfs:range rdf:resource="http://www.w3.org/2001/XMLSchema#string"/>
  </owl:DatatypeProperty>
  <owl:DatatypeProperty rdf:about="http://example.org/onto/prop/yandex_iam_service_account_update">
    <rdfs:label>update</rdfs:label>
    <rdfs:comment>A string that can be [parsed as a duration](https://pkg.go.dev/time#ParseDuration) consisting of numbers and unit suffixes, such as "30s" or "2h45m". Valid time units are "s" (seconds), "m" (minutes), "h" (hours).</rdfs:comment>
    <rdfs:domain rdf:resource="http://example.org/onto/class/yandex_iam_service_account"/>
    <rdfs:range rdf:resource="http://www.w3.org/2001/XMLSchema#string"/>
  </owl:DatatypeProperty>
</rdf:RDF>
