<?xml version="1.0" encoding="UTF-8"?>
<rdf:RDF
  xmlns:rdf="http://www.w3.org/1999/02/22-rdf-syntax-ns#"
  xmlns:rdfs="http://www.w3.org/2000/01/rdf-schema#"
  xmlns:owl="http://www.w3.org/2002/07/owl#"
  xmlns:xsd="http://www.w3.org/2001/XMLSchema#"
  xml:base="http://example.org/onto/">
  <owl:Class rdf:about="http://example.org/onto/class/yandex_compute_filesystem">
    <rdfs:label>yandex_compute_filesystem</rdfs:label>
    <rdfs:comment>A filesystem resource.
 For details about the concept, see [documentation](/docs/compute/concepts/filesystem).</rdfs:comment>
  </owl:Class>
  <owl:DatatypeProperty rdf:about="http://example.org/onto/prop/yandex_compute_filesystem_block_size">
    <rdfs:label>block_size</rdfs:label>
    <rdfs:comment>Block size used for the filesystem, specified in bytes.</rdfs:comment>
    <rdfs:domain rdf:resource="http://example.org/onto/class/yandex_compute_filesystem"/>
    <rdfs:range rdf:resource="http://www.w3.org/2001/XMLSchema#string"/>
  </owl:DatatypeProperty>
  <owl:DatatypeProperty rdf:about="http://example.org/onto/prop/yandex_compute_filesystem_created_at">
    <rdfs:label>created_at</rdfs:label>
    <rdfs:comment>Creation timestamp.</rdfs:comment>
    <rdfs:domain rdf:resource="http://example.org/onto/class/yandex_compute_filesystem"/>
    <rdfs:range rdf:resource="http://www.w3.org/2001/XMLSchema#string"/>
  </owl:DatatypeProperty>
  <owl:DatatypeProperty rdf:about="http://example.org/onto/prop/yandex_compute_filesystem_description">
    <rdfs:label>description</rdfs:label>
    <rdfs:comment>Description of the filesystem.</rdfs:comment>
    <rdfs:domain rdf:resource="http://example.org/onto/class/yandex_compute_filesystem"/>
    <rdfs:range rdf:resource="http://www.w3.org/2001/XMLSchema#string"/>
  </owl:DatatypeProperty>
  <owl:DatatypeProperty rdf:about="http://example.org/onto/prop/yandex_compute_filesystem_filesystem_id">
    <rdfs:label>filesystem_id</rdfs:label>
    <rdfs:comment>ID of the filesystem to return.

 To get the filesystem ID, make a [FilesystemService.List] request.</rdfs:comment>
    <rdfs:domain rdf:resource="http://example.org/onto/class/yandex_compute_filesystem"/>
    <rdfs:range rdf:resource="http://www.w3.org/2001/XMLSchema#string"/>
  </owl:DatatypeProperty>
  <owl:DatatypeProperty rdf:about="http://example.org/onto/prop/yandex_compute_filesystem_folder_id">
    <rdfs:label>folder_id</rdfs:label>
    <rdfs:comment>ID of the folder that the filesystem belongs to.</rdfs:comment>
    <rdfs:domain rdf:resource="http://example.org/onto/class/yandex_compute_filesystem"/>
    <rdfs:range rdf:resource="http://www.w3.org/2001/XMLSchema#string"/>
  </owl:DatatypeProperty>
  <owl:DatatypeProperty rdf:about="http://example.org/onto/prop/yandex_compute_filesystem_id">
    <rdfs:label>id</rdfs:label>
    <rdfs:comment>ID of the filesystem to return.

 To get the filesystem ID, make a [FilesystemService.List] request.</rdfs:comment>
    <rdfs:domain rdf:resource="http://example.org/onto/class/yandex_compute_filesystem"/>
    <rdfs:range rdf:resource="http://www.w3.org/2001/XMLSchema#string"/>
  </owl:DatatypeProperty>
  <owl:DatatypeProperty rdf:about="http://example.org/onto/prop/yandex_compute_filesystem_labels">
    <rdfs:label>labels</rdfs:label>
    <rdfs:comment>Filesystem labels as `key:value` pairs.
 For details about the concept, see [documentation](/docs/overview/concepts/services#labels).</rdfs:comment>
    <rdfs:domain rdf:resource="http://example.org/onto/class/yandex_compute_filesystem"/>
    <rdfs:range rdf:resource="http://www.w3.org/2001/XMLSchema#string"/>
  </owl:DatatypeProperty>
  <owl:DatatypeProperty rdf:about="http://example.org/onto/prop/yandex_compute_filesystem_name">
    <rdfs:label>name</rdfs:label>
    <rdfs:comment>Name of the filesystem. The name is unique within the folder.</rdfs:comment>
    <rdfs:domain rdf:resource="http://example.org/onto/class/yandex_compute_filesystem"/>
    <rdfs:range rdf:resource="http://www.w3.org/2001/XMLSchema#string"/>
  </owl:DatatypeProperty>
  <owl:DatatypeProperty rdf:about="http://example.org/onto/prop/yandex_compute_filesystem_size">
    <rdfs:label>size</rdfs:label>
    <rdfs:comment>Size of the filesystem, specified in bytes.</rdfs:comment>
    <rdfs:domain rdf:resource="http://example.org/onto/class/yandex_compute_filesystem"/>
    <rdfs:range rdf:resource="http://www.w3.org/2001/XMLSchema#string"/>
  </owl:DatatypeProperty>
  <owl:DatatypeProperty rdf:about="http://example.org/onto/prop/yandex_compute_filesystem_status">
    <rdfs:label>status</rdfs:label>
    <rdfs:comment>Current status of the filesystem.</rdfs:comment>
    <rdfs:domain rdf:resource="http://example.org/onto/class/yandex_compute_filesystem"/>
    <rdfs:range rdf:resource="http://www.w3.org/2001/XMLSchema#string"/>
  </owl:DatatypeProperty>
  <owl:DatatypeProperty rdf:about="http://example.org/onto/prop/yandex_compute_filesystem_type">
    <rdfs:label>type</rdfs:label>
    <rdfs:comment>ID of the filesystem type.

 To get a list of available filesystem types, make a [yandex.cloud.compute.v1.DiskTypeService.List] request.</rdfs:comment>
    <rdfs:domain rdf:resource="http://example.org/onto/class/yandex_compute_filesystem"/>
    <rdfs:range rdf:resource="http://www.w3.org/2001/XMLSchema#string"/>
  </owl:DatatypeProperty>
  <owl:DatatypeProperty rdf:about="http://example.org/onto/prop/yandex_compute_filesystem_zone">
    <rdfs:label>zone</rdfs:label>
    <rdfs:comment>ID of the availability zone where the filesystem resides.

 A filesystem can be attached only to instances residing in the same availability zone.</rdfs:comment>
    <rdfs:domain rdf:resource="http://example.org/onto/class/yandex_compute_filesystem"/>
    <rdfs:range rdf:resource="http://www.w3.org/2001/XMLSchema#string"/>
  </owl:DatatypeProperty>
  <owl:DatatypeProperty rdf:about="http://example.org/onto/prop/yandex_compute_filesystem_create">
    <rdfs:label>create</rdfs:label>
    <rdfs:comment>A string that can be [parsed as a duration](https://pkg.go.dev/time#ParseDuration) consisting of numbers and unit suffixes, such as "30s" or "2h45m". Valid time units are "s" (seconds), "m" (minutes), "h" (hours).</rdfs:comment>
    <rdfs:domain rdf:resource="http://example.org/onto/class/yandex_compute_filesystem"/>
    <rdfs:range rdf:resource="http://www.w3.org/2001/XMLSchema#string"/>
  </owl:DatatypeProperty>
  <owl:DatatypeProperty rdf:about="http://example.org/onto/prop/yandex_compute_filesystem_delete">
    <rdfs:label>delete</rdfs:label>
    <rdfs:comment>A string that can be [parsed as a duration](https://pkg.go.dev/time#ParseDuration) consisting of numbers and unit suffixes, such as "30s" or "2h45m". Valid time units are "s" (seconds), "m" (minutes), "h" (hours). Setting a timeout for a Delete operation is only applicable if changes are saved into state before the destroy operation occurs.</rdfs:comment>
    <rdfs:domain rdf:resource="http://example.org/onto/class/yandex_compute_filesystem"/>
    <rdfs:range rdf:resource="http://www.w3.org/2001/XMLSchema#string"/>
  </owl:DatatypeProperty>
  <owl:DatatypeProperty rdf:about="http://example.org/onto/prop/yandex_compute_filesystem_read">
    <rdfs:label>read</rdfs:label>
    <rdfs:comment>A string that can be [parsed as a duration](https://pkg.go.dev/time#ParseDuration) consisting of numbers and unit suffixes, such as "30s" or "2h45m". Valid time units are "s" (seconds), "m" (minutes), "h" (hours). Read operations occur during any refresh or planning operation when refresh is enabled.</rdfs:comment>
    <rdfs:domain rdf:resource="http://example.org/onto/class/yandex_compute_filesystem"/>
    <rdfs:range rdf:resource="http://www.w3.org/2001/XMLSchema#string"/>
  </owl:DatatypeProperty>
  <owl:DatatypeProperty rdf:about="http://example.org/onto/prop/yandex_compute_filesystem_update">
    <rdfs:label>update</rdfs:label>
    <rdfs:comment>A string that can be [parsed as a duration](https://pkg.go.dev/time#ParseDuration) consisting of numbers and unit suffixes, such as "30s" or "2h45m". Valid time units are "s" (seconds), "m" (minutes), "h" (hours).</rdfs:comment>
    <rdfs:domain rdf:resource="http://example.org/onto/class/yandex_compute_filesystem"/>
    <rdfs:range rdf:resource="http://www.w3.org/2001/XMLSchema#string"/>
  </owl:DatatypeProperty>
</rdf:RDF>
