<?xml version="1.0" encoding="UTF-8"?>
<rdf:RDF
  xmlns:rdf="http://www.w3.org/1999/02/22-rdf-syntax-ns#"
  xmlns:rdfs="http://www.w3.org/2000/01/rdf-schema#"
  xmlns:owl="http://www.w3.org/2002/07/owl#"
  xmlns:xsd="http://www.w3.org/2001/XMLSchema#"
  xml:base="http://example.org/onto/">
  <owl:Class rdf:about="http://example.org/onto/class/yandex_mdb_postgresql_cluster">
    <rdfs:label>yandex_mdb_postgresql_cluster</rdfs:label>
    <rdfs:comment>Manages a PostgreSQL cluster within the Yandex Cloud. For more information, see [the official documentation](https://yandex.cloud/docs/managed-postgresql/). [How to connect to the DB](https://yandex.cloud/docs/managed-postgresql/quickstart#connect). To connect, use port 6432. The port number is not configurable.

~> Historically, `user` and `database` blocks of the `yandex_mdb_postgresql_cluster` resource were used to manage users and databases of the PostgreSQL cluster. However, this approach has many disadvantages. In particular, adding and removing a resource from the terraform recipe worked wrong because terraform misleads the user about the planned changes. Now, the recommended way to manage databases and users is using `yandex_mdb_postgresql_user` and `yandex_mdb_postgresql_database` resources.</rdfs:comment>
  </owl:Class>
  <owl:DatatypeProperty rdf:about="http://example.org/onto/prop/yandex_mdb_postgresql_cluster_created_at">
    <rdfs:label>created_at</rdfs:label>
    <rdfs:comment>The creation timestamp of the resource.</rdfs:comment>
    <rdfs:domain rdf:resource="http://example.org/onto/class/yandex_mdb_postgresql_cluster"/>
    <rdfs:range rdf:resource="http://www.w3.org/2001/XMLSchema#string"/>
  </owl:DatatypeProperty>
  <owl:DatatypeProperty rdf:about="http://example.org/onto/prop/yandex_mdb_postgresql_cluster_deletion_protection">
    <rdfs:label>deletion_protection</rdfs:label>
    <rdfs:comment>The `true` value means that resource is protected from accidental deletion.</rdfs:comment>
    <rdfs:domain rdf:resource="http://example.org/onto/class/yandex_mdb_postgresql_cluster"/>
    <rdfs:range rdf:resource="http://www.w3.org/2001/XMLSchema#string"/>
  </owl:DatatypeProperty>
  <owl:DatatypeProperty rdf:about="http://example.org/onto/prop/yandex_mdb_postgresql_cluster_description">
    <rdfs:label>description</rdfs:label>
    <rdfs:comment>The resource description.</rdfs:comment>
    <rdfs:domain rdf:resource="http://example.org/onto/class/yandex_mdb_postgresql_cluster"/>
    <rdfs:range rdf:resource="http://www.w3.org/2001/XMLSchema#string"/>
  </owl:DatatypeProperty>
  <owl:DatatypeProperty rdf:about="http://example.org/onto/prop/yandex_mdb_postgresql_cluster_disk_encryption_key_id">
    <rdfs:label>disk_encryption_key_id</rdfs:label>
    <rdfs:comment>ID of the KMS key for cluster disk encryption. Restoring without an encryption key will disable encryption if any exists.</rdfs:comment>
    <rdfs:domain rdf:resource="http://example.org/onto/class/yandex_mdb_postgresql_cluster"/>
    <rdfs:range rdf:resource="http://www.w3.org/2001/XMLSchema#string"/>
  </owl:DatatypeProperty>
  <owl:DatatypeProperty rdf:about="http://example.org/onto/prop/yandex_mdb_postgresql_cluster_environment">
    <rdfs:label>environment</rdfs:label>
    <rdfs:comment>Deployment environment of the PostgreSQL cluster.</rdfs:comment>
    <rdfs:domain rdf:resource="http://example.org/onto/class/yandex_mdb_postgresql_cluster"/>
    <rdfs:range rdf:resource="http://www.w3.org/2001/XMLSchema#string"/>
  </owl:DatatypeProperty>
  <owl:DatatypeProperty rdf:about="http://example.org/onto/prop/yandex_mdb_postgresql_cluster_folder_id">
    <rdfs:label>folder_id</rdfs:label>
    <rdfs:comment>The folder identifier that resource belongs to. If it is not provided, the default provider `folder-id` is used.</rdfs:comment>
    <rdfs:domain rdf:resource="http://example.org/onto/class/yandex_mdb_postgresql_cluster"/>
    <rdfs:range rdf:resource="http://www.w3.org/2001/XMLSchema#string"/>
  </owl:DatatypeProperty>
  <owl:DatatypeProperty rdf:about="http://example.org/onto/prop/yandex_mdb_postgresql_cluster_health">
    <rdfs:label>health</rdfs:label>
    <rdfs:comment>Aggregated health of the cluster.</rdfs:comment>
    <rdfs:domain rdf:resource="http://example.org/onto/class/yandex_mdb_postgresql_cluster"/>
    <rdfs:range rdf:resource="http://www.w3.org/2001/XMLSchema#string"/>
  </owl:DatatypeProperty>
  <owl:DatatypeProperty rdf:about="http://example.org/onto/prop/yandex_mdb_postgresql_cluster_host_group_ids">
    <rdfs:label>host_group_ids</rdfs:label>
    <rdfs:comment>Host Group IDs.</rdfs:comment>
    <rdfs:domain rdf:resource="http://example.org/onto/class/yandex_mdb_postgresql_cluster"/>
    <rdfs:range rdf:resource="http://www.w3.org/2001/XMLSchema#string"/>
  </owl:DatatypeProperty>
  <owl:DatatypeProperty rdf:about="http://example.org/onto/prop/yandex_mdb_postgresql_cluster_host_master_name">
    <rdfs:label>host_master_name</rdfs:label>
    <rdfs:comment>Deprecated field. Will be removed in future versions.</rdfs:comment>
    <rdfs:domain rdf:resource="http://example.org/onto/class/yandex_mdb_postgresql_cluster"/>
    <rdfs:range rdf:resource="http://www.w3.org/2001/XMLSchema#string"/>
  </owl:DatatypeProperty>
  <owl:DatatypeProperty rdf:about="http://example.org/onto/prop/yandex_mdb_postgresql_cluster_id">
    <rdfs:label>id</rdfs:label>
    <rdfs:domain rdf:resource="http://example.org/onto/class/yandex_mdb_postgresql_cluster"/>
    <rdfs:range rdf:resource="http://www.w3.org/2001/XMLSchema#string"/>
  </owl:DatatypeProperty>
  <owl:DatatypeProperty rdf:about="http://example.org/onto/prop/yandex_mdb_postgresql_cluster_labels">
    <rdfs:label>labels</rdfs:label>
    <rdfs:comment>A set of key/value label pairs which assigned to resource.</rdfs:comment>
    <rdfs:domain rdf:resource="http://example.org/onto/class/yandex_mdb_postgresql_cluster"/>
    <rdfs:range rdf:resource="http://www.w3.org/2001/XMLSchema#string"/>
  </owl:DatatypeProperty>
  <owl:DatatypeProperty rdf:about="http://example.org/onto/prop/yandex_mdb_postgresql_cluster_name">
    <rdfs:label>name</rdfs:label>
    <rdfs:comment>The resource name.</rdfs:comment>
    <rdfs:domain rdf:resource="http://example.org/onto/class/yandex_mdb_postgresql_cluster"/>
    <rdfs:range rdf:resource="http://www.w3.org/2001/XMLSchema#string"/>
  </owl:DatatypeProperty>
  <owl:DatatypeProperty rdf:about="http://example.org/onto/prop/yandex_mdb_postgresql_cluster_network_id">
    <rdfs:label>network_id</rdfs:label>
    <rdfs:comment>The `VPC Network ID` of subnets which resource attached to.</rdfs:comment>
    <rdfs:domain rdf:resource="http://example.org/onto/class/yandex_mdb_postgresql_cluster"/>
    <rdfs:range rdf:resource="http://www.w3.org/2001/XMLSchema#string"/>
  </owl:DatatypeProperty>
  <owl:DatatypeProperty rdf:about="http://example.org/onto/prop/yandex_mdb_postgresql_cluster_security_group_ids">
    <rdfs:label>security_group_ids</rdfs:label>
    <rdfs:comment>The list of security groups applied to resource or their components.</rdfs:comment>
    <rdfs:domain rdf:resource="http://example.org/onto/class/yandex_mdb_postgresql_cluster"/>
    <rdfs:range rdf:resource="http://www.w3.org/2001/XMLSchema#string"/>
  </owl:DatatypeProperty>
  <owl:DatatypeProperty rdf:about="http://example.org/onto/prop/yandex_mdb_postgresql_cluster_status">
    <rdfs:label>status</rdfs:label>
    <rdfs:comment>Status of the cluster.</rdfs:comment>
    <rdfs:domain rdf:resource="http://example.org/onto/class/yandex_mdb_postgresql_cluster"/>
    <rdfs:range rdf:resource="http://www.w3.org/2001/XMLSchema#string"/>
  </owl:DatatypeProperty>
  <owl:DatatypeProperty rdf:about="http://example.org/onto/prop/yandex_mdb_postgresql_cluster_autofailover">
    <rdfs:label>autofailover</rdfs:label>
    <rdfs:comment>Configuration setting which enables/disables autofailover in cluster.</rdfs:comment>
    <rdfs:domain rdf:resource="http://example.org/onto/class/yandex_mdb_postgresql_cluster"/>
    <rdfs:range rdf:resource="http://www.w3.org/2001/XMLSchema#string"/>
  </owl:DatatypeProperty>
  <owl:DatatypeProperty rdf:about="http://example.org/onto/prop/yandex_mdb_postgresql_cluster_backup_retain_period_days">
    <rdfs:label>backup_retain_period_days</rdfs:label>
    <rdfs:comment>The period in days during which backups are stored.</rdfs:comment>
    <rdfs:domain rdf:resource="http://example.org/onto/class/yandex_mdb_postgresql_cluster"/>
    <rdfs:range rdf:resource="http://www.w3.org/2001/XMLSchema#string"/>
  </owl:DatatypeProperty>
  <owl:DatatypeProperty rdf:about="http://example.org/onto/prop/yandex_mdb_postgresql_cluster_postgresql_config">
    <rdfs:label>postgresql_config</rdfs:label>
    <rdfs:comment>PostgreSQL cluster configuration. For detailed information specific to your PostgreSQL version, please refer to the [API proto specifications](https://github.com/yandex-cloud/cloudapi/tree/master/yandex/cloud/mdb/postgresql/v1/config).</rdfs:comment>
    <rdfs:domain rdf:resource="http://example.org/onto/class/yandex_mdb_postgresql_cluster"/>
    <rdfs:range rdf:resource="http://www.w3.org/2001/XMLSchema#string"/>
  </owl:DatatypeProperty>
  <owl:DatatypeProperty rdf:about="http://example.org/onto/prop/yandex_mdb_postgresql_cluster_version">
    <rdfs:label>version</rdfs:label>
    <rdfs:comment>Version of the PostgreSQL cluster. (allowed versions are: 13, 13-1c, 14, 14-1c, 15, 15-1c, 16, 17).</rdfs:comment>
    <rdfs:domain rdf:resource="http://example.org/onto/class/yandex_mdb_postgresql_cluster"/>
    <rdfs:range rdf:resource="http://www.w3.org/2001/XMLSchema#string"/>
  </owl:DatatypeProperty>
  <owl:DatatypeProperty rdf:about="http://example.org/onto/prop/yandex_mdb_postgresql_cluster_data_lens">
    <rdfs:label>data_lens</rdfs:label>
    <rdfs:comment>Allow access for [Yandex DataLens](https://yandex.cloud/services/datalens).</rdfs:comment>
    <rdfs:domain rdf:resource="http://example.org/onto/class/yandex_mdb_postgresql_cluster"/>
    <rdfs:range rdf:resource="http://www.w3.org/2001/XMLSchema#string"/>
  </owl:DatatypeProperty>
  <owl:DatatypeProperty rdf:about="http://example.org/onto/prop/yandex_mdb_postgresql_cluster_data_transfer">
    <rdfs:label>data_transfer</rdfs:label>
    <rdfs:comment>Allow access for [DataTransfer](https://yandex.cloud/services/data-transfer).</rdfs:comment>
    <rdfs:domain rdf:resource="http://example.org/onto/class/yandex_mdb_postgresql_cluster"/>
    <rdfs:range rdf:resource="http://www.w3.org/2001/XMLSchema#string"/>
  </owl:DatatypeProperty>
  <owl:DatatypeProperty rdf:about="http://example.org/onto/prop/yandex_mdb_postgresql_cluster_serverless">
    <rdfs:label>serverless</rdfs:label>
    <rdfs:comment>Allow access for [connection to managed databases from functions](https://yandex.cloud/docs/functions/operations/database-connection).</rdfs:comment>
    <rdfs:domain rdf:resource="http://example.org/onto/class/yandex_mdb_postgresql_cluster"/>
    <rdfs:range rdf:resource="http://www.w3.org/2001/XMLSchema#string"/>
  </owl:DatatypeProperty>
  <owl:DatatypeProperty rdf:about="http://example.org/onto/prop/yandex_mdb_postgresql_cluster_web_sql">
    <rdfs:label>web_sql</rdfs:label>
    <rdfs:comment>Allow access for [SQL queries in the management console](https://yandex.cloud/docs/managed-postgresql/operations/web-sql-query).</rdfs:comment>
    <rdfs:domain rdf:resource="http://example.org/onto/class/yandex_mdb_postgresql_cluster"/>
    <rdfs:range rdf:resource="http://www.w3.org/2001/XMLSchema#string"/>
  </owl:DatatypeProperty>
  <owl:DatatypeProperty rdf:about="http://example.org/onto/prop/yandex_mdb_postgresql_cluster_hours">
    <rdfs:label>hours</rdfs:label>
    <rdfs:comment>The hour at which backup will be started (UTC).</rdfs:comment>
    <rdfs:domain rdf:resource="http://example.org/onto/class/yandex_mdb_postgresql_cluster"/>
    <rdfs:range rdf:resource="http://www.w3.org/2001/XMLSchema#string"/>
  </owl:DatatypeProperty>
  <owl:DatatypeProperty rdf:about="http://example.org/onto/prop/yandex_mdb_postgresql_cluster_minutes">
    <rdfs:label>minutes</rdfs:label>
    <rdfs:comment>The minute at which backup will be started.</rdfs:comment>
    <rdfs:domain rdf:resource="http://example.org/onto/class/yandex_mdb_postgresql_cluster"/>
    <rdfs:range rdf:resource="http://www.w3.org/2001/XMLSchema#string"/>
  </owl:DatatypeProperty>
  <owl:DatatypeProperty rdf:about="http://example.org/onto/prop/yandex_mdb_postgresql_cluster_disk_size_limit">
    <rdfs:label>disk_size_limit</rdfs:label>
    <rdfs:comment>The overall maximum for disk size that limit all autoscaling iterations. See the [documentation](https://yandex.cloud/en/docs/managed-postgresql/concepts/storage#auto-rescale) for details.</rdfs:comment>
    <rdfs:domain rdf:resource="http://example.org/onto/class/yandex_mdb_postgresql_cluster"/>
    <rdfs:range rdf:resource="http://www.w3.org/2001/XMLSchema#string"/>
  </owl:DatatypeProperty>
  <owl:DatatypeProperty rdf:about="http://example.org/onto/prop/yandex_mdb_postgresql_cluster_emergency_usage_threshold">
    <rdfs:label>emergency_usage_threshold</rdfs:label>
    <rdfs:comment>Threshold of storage usage (in percent) that triggers immediate automatic scaling of the storage. Zero value means disabled threshold.</rdfs:comment>
    <rdfs:domain rdf:resource="http://example.org/onto/class/yandex_mdb_postgresql_cluster"/>
    <rdfs:range rdf:resource="http://www.w3.org/2001/XMLSchema#string"/>
  </owl:DatatypeProperty>
  <owl:DatatypeProperty rdf:about="http://example.org/onto/prop/yandex_mdb_postgresql_cluster_planned_usage_threshold">
    <rdfs:label>planned_usage_threshold</rdfs:label>
    <rdfs:comment>Threshold of storage usage (in percent) that triggers automatic scaling of the storage during the maintenance window. Zero value means disabled threshold.</rdfs:comment>
    <rdfs:domain rdf:resource="http://example.org/onto/class/yandex_mdb_postgresql_cluster"/>
    <rdfs:range rdf:resource="http://www.w3.org/2001/XMLSchema#string"/>
  </owl:DatatypeProperty>
  <owl:DatatypeProperty rdf:about="http://example.org/onto/prop/yandex_mdb_postgresql_cluster_enabled">
    <rdfs:label>enabled</rdfs:label>
    <rdfs:comment>Enable performance diagnostics.</rdfs:comment>
    <rdfs:domain rdf:resource="http://example.org/onto/class/yandex_mdb_postgresql_cluster"/>
    <rdfs:range rdf:resource="http://www.w3.org/2001/XMLSchema#string"/>
  </owl:DatatypeProperty>
  <owl:DatatypeProperty rdf:about="http://example.org/onto/prop/yandex_mdb_postgresql_cluster_sessions_sampling_interval">
    <rdfs:label>sessions_sampling_interval</rdfs:label>
    <rdfs:comment>Interval (in seconds) for pg_stat_activity sampling. Acceptable values are 1 to 86400, inclusive.</rdfs:comment>
    <rdfs:domain rdf:resource="http://example.org/onto/class/yandex_mdb_postgresql_cluster"/>
    <rdfs:range rdf:resource="http://www.w3.org/2001/XMLSchema#string"/>
  </owl:DatatypeProperty>
  <owl:DatatypeProperty rdf:about="http://example.org/onto/prop/yandex_mdb_postgresql_cluster_statements_sampling_interval">
    <rdfs:label>statements_sampling_interval</rdfs:label>
    <rdfs:comment>Interval (in seconds) for pg_stat_statements sampling. Acceptable values are 1 to 86400, inclusive.</rdfs:comment>
    <rdfs:domain rdf:resource="http://example.org/onto/class/yandex_mdb_postgresql_cluster"/>
    <rdfs:range rdf:resource="http://www.w3.org/2001/XMLSchema#string"/>
  </owl:DatatypeProperty>
  <owl:DatatypeProperty rdf:about="http://example.org/onto/prop/yandex_mdb_postgresql_cluster_pool_discard">
    <rdfs:label>pool_discard</rdfs:label>
    <rdfs:comment>Setting `pool_discard` [parameter in Odyssey](https://github.com/yandex/odyssey/blob/master/documentation/configuration.md#pool_discard-yesno).</rdfs:comment>
    <rdfs:domain rdf:resource="http://example.org/onto/class/yandex_mdb_postgresql_cluster"/>
    <rdfs:range rdf:resource="http://www.w3.org/2001/XMLSchema#string"/>
  </owl:DatatypeProperty>
  <owl:DatatypeProperty rdf:about="http://example.org/onto/prop/yandex_mdb_postgresql_cluster_pooling_mode">
    <rdfs:label>pooling_mode</rdfs:label>
    <rdfs:comment>Mode that the connection pooler is working in. See descriptions of all modes in the [documentation for Odyssey](https://github.com/yandex/odyssey/blob/master/documentation/configuration.md#pool-string.</rdfs:comment>
    <rdfs:domain rdf:resource="http://example.org/onto/class/yandex_mdb_postgresql_cluster"/>
    <rdfs:range rdf:resource="http://www.w3.org/2001/XMLSchema#string"/>
  </owl:DatatypeProperty>
  <owl:DatatypeProperty rdf:about="http://example.org/onto/prop/yandex_mdb_postgresql_cluster_disk_size">
    <rdfs:label>disk_size</rdfs:label>
    <rdfs:comment>Volume of the storage available to a PostgreSQL host, in gigabytes.</rdfs:comment>
    <rdfs:domain rdf:resource="http://example.org/onto/class/yandex_mdb_postgresql_cluster"/>
    <rdfs:range rdf:resource="http://www.w3.org/2001/XMLSchema#string"/>
  </owl:DatatypeProperty>
  <owl:DatatypeProperty rdf:about="http://example.org/onto/prop/yandex_mdb_postgresql_cluster_disk_type_id">
    <rdfs:label>disk_type_id</rdfs:label>
    <rdfs:comment>Type of the storage of PostgreSQL hosts.</rdfs:comment>
    <rdfs:domain rdf:resource="http://example.org/onto/class/yandex_mdb_postgresql_cluster"/>
    <rdfs:range rdf:resource="http://www.w3.org/2001/XMLSchema#string"/>
  </owl:DatatypeProperty>
  <owl:DatatypeProperty rdf:about="http://example.org/onto/prop/yandex_mdb_postgresql_cluster_resource_preset_id">
    <rdfs:label>resource_preset_id</rdfs:label>
    <rdfs:comment>The ID of the preset for computational resources available to a PostgreSQL host (CPU, memory etc.). For more information, see [the official documentation](https://yandex.cloud/docs/managed-postgresql/concepts/instance-types).</rdfs:comment>
    <rdfs:domain rdf:resource="http://example.org/onto/class/yandex_mdb_postgresql_cluster"/>
    <rdfs:range rdf:resource="http://www.w3.org/2001/XMLSchema#string"/>
  </owl:DatatypeProperty>
  <owl:DatatypeProperty rdf:about="http://example.org/onto/prop/yandex_mdb_postgresql_cluster_lc_collate">
    <rdfs:label>lc_collate</rdfs:label>
    <rdfs:comment>POSIX locale for string sorting order. Forbidden to change in an existing database.</rdfs:comment>
    <rdfs:domain rdf:resource="http://example.org/onto/class/yandex_mdb_postgresql_cluster"/>
    <rdfs:range rdf:resource="http://www.w3.org/2001/XMLSchema#string"/>
  </owl:DatatypeProperty>
  <owl:DatatypeProperty rdf:about="http://example.org/onto/prop/yandex_mdb_postgresql_cluster_lc_type">
    <rdfs:label>lc_type</rdfs:label>
    <rdfs:comment>POSIX locale for character classification. Forbidden to change in an existing database.</rdfs:comment>
    <rdfs:domain rdf:resource="http://example.org/onto/class/yandex_mdb_postgresql_cluster"/>
    <rdfs:range rdf:resource="http://www.w3.org/2001/XMLSchema#string"/>
  </owl:DatatypeProperty>
  <owl:DatatypeProperty rdf:about="http://example.org/onto/prop/yandex_mdb_postgresql_cluster_name">
    <rdfs:label>name</rdfs:label>
    <rdfs:comment>The resource name.</rdfs:comment>
    <rdfs:domain rdf:resource="http://example.org/onto/class/yandex_mdb_postgresql_cluster"/>
    <rdfs:range rdf:resource="http://www.w3.org/2001/XMLSchema#string"/>
  </owl:DatatypeProperty>
  <owl:DatatypeProperty rdf:about="http://example.org/onto/prop/yandex_mdb_postgresql_cluster_owner">
    <rdfs:label>owner</rdfs:label>
    <rdfs:comment>Name of the user assigned as the owner of the database. Forbidden to change in an existing database.</rdfs:comment>
    <rdfs:domain rdf:resource="http://example.org/onto/class/yandex_mdb_postgresql_cluster"/>
    <rdfs:range rdf:resource="http://www.w3.org/2001/XMLSchema#string"/>
  </owl:DatatypeProperty>
  <owl:DatatypeProperty rdf:about="http://example.org/onto/prop/yandex_mdb_postgresql_cluster_template_db">
    <rdfs:label>template_db</rdfs:label>
    <rdfs:comment>Name of the template database.</rdfs:comment>
    <rdfs:domain rdf:resource="http://example.org/onto/class/yandex_mdb_postgresql_cluster"/>
    <rdfs:range rdf:resource="http://www.w3.org/2001/XMLSchema#string"/>
  </owl:DatatypeProperty>
  <owl:DatatypeProperty rdf:about="http://example.org/onto/prop/yandex_mdb_postgresql_cluster_name">
    <rdfs:label>name</rdfs:label>
    <rdfs:comment>Name of the database extension. For more information on available extensions see [the official documentation](https://yandex.cloud/docs/managed-postgresql/operations/cluster-extensions).</rdfs:comment>
    <rdfs:domain rdf:resource="http://example.org/onto/class/yandex_mdb_postgresql_cluster"/>
    <rdfs:range rdf:resource="http://www.w3.org/2001/XMLSchema#string"/>
  </owl:DatatypeProperty>
  <owl:DatatypeProperty rdf:about="http://example.org/onto/prop/yandex_mdb_postgresql_cluster_version">
    <rdfs:label>version</rdfs:label>
    <rdfs:comment>Version of the extension.</rdfs:comment>
    <rdfs:domain rdf:resource="http://example.org/onto/class/yandex_mdb_postgresql_cluster"/>
    <rdfs:range rdf:resource="http://www.w3.org/2001/XMLSchema#string"/>
  </owl:DatatypeProperty>
  <owl:DatatypeProperty rdf:about="http://example.org/onto/prop/yandex_mdb_postgresql_cluster_assign_public_ip">
    <rdfs:label>assign_public_ip</rdfs:label>
    <rdfs:comment>Whether the host should get a public IP address.</rdfs:comment>
    <rdfs:domain rdf:resource="http://example.org/onto/class/yandex_mdb_postgresql_cluster"/>
    <rdfs:range rdf:resource="http://www.w3.org/2001/XMLSchema#string"/>
  </owl:DatatypeProperty>
  <owl:DatatypeProperty rdf:about="http://example.org/onto/prop/yandex_mdb_postgresql_cluster_fqdn">
    <rdfs:label>fqdn</rdfs:label>
    <rdfs:comment>The fully qualified domain name of the host.</rdfs:comment>
    <rdfs:domain rdf:resource="http://example.org/onto/class/yandex_mdb_postgresql_cluster"/>
    <rdfs:range rdf:resource="http://www.w3.org/2001/XMLSchema#string"/>
  </owl:DatatypeProperty>
  <owl:DatatypeProperty rdf:about="http://example.org/onto/prop/yandex_mdb_postgresql_cluster_name">
    <rdfs:label>name</rdfs:label>
    <rdfs:comment>Host state name. It should be set for all hosts or unset for all hosts. This field can be used by another host, to select which host will be its replication source. Please see `replication_source_name` parameter.</rdfs:comment>
    <rdfs:domain rdf:resource="http://example.org/onto/class/yandex_mdb_postgresql_cluster"/>
    <rdfs:range rdf:resource="http://www.w3.org/2001/XMLSchema#string"/>
  </owl:DatatypeProperty>
  <owl:DatatypeProperty rdf:about="http://example.org/onto/prop/yandex_mdb_postgresql_cluster_priority">
    <rdfs:label>priority</rdfs:label>
    <rdfs:comment>Host priority in HA group. It works only when `name` is set.</rdfs:comment>
    <rdfs:domain rdf:resource="http://example.org/onto/class/yandex_mdb_postgresql_cluster"/>
    <rdfs:range rdf:resource="http://www.w3.org/2001/XMLSchema#string"/>
  </owl:DatatypeProperty>
  <owl:DatatypeProperty rdf:about="http://example.org/onto/prop/yandex_mdb_postgresql_cluster_replication_source">
    <rdfs:label>replication_source</rdfs:label>
    <rdfs:comment>Host replication source (fqdn), when replication_source is empty then host is in HA group.</rdfs:comment>
    <rdfs:domain rdf:resource="http://example.org/onto/class/yandex_mdb_postgresql_cluster"/>
    <rdfs:range rdf:resource="http://www.w3.org/2001/XMLSchema#string"/>
  </owl:DatatypeProperty>
  <owl:DatatypeProperty rdf:about="http://example.org/onto/prop/yandex_mdb_postgresql_cluster_replication_source_name">
    <rdfs:label>replication_source_name</rdfs:label>
    <rdfs:comment>Host replication source name points to host's `name` from which this host should replicate. When not set then host in HA group. It works only when `name` is set.</rdfs:comment>
    <rdfs:domain rdf:resource="http://example.org/onto/class/yandex_mdb_postgresql_cluster"/>
    <rdfs:range rdf:resource="http://www.w3.org/2001/XMLSchema#string"/>
  </owl:DatatypeProperty>
  <owl:DatatypeProperty rdf:about="http://example.org/onto/prop/yandex_mdb_postgresql_cluster_role">
    <rdfs:label>role</rdfs:label>
    <rdfs:comment>Host's role (replica|primary), computed by server.</rdfs:comment>
    <rdfs:domain rdf:resource="http://example.org/onto/class/yandex_mdb_postgresql_cluster"/>
    <rdfs:range rdf:resource="http://www.w3.org/2001/XMLSchema#string"/>
  </owl:DatatypeProperty>
  <owl:DatatypeProperty rdf:about="http://example.org/onto/prop/yandex_mdb_postgresql_cluster_subnet_id">
    <rdfs:label>subnet_id</rdfs:label>
    <rdfs:comment>The ID of the subnet, to which the host belongs. The subnet must be a part of the network to which the cluster belongs.</rdfs:comment>
    <rdfs:domain rdf:resource="http://example.org/onto/class/yandex_mdb_postgresql_cluster"/>
    <rdfs:range rdf:resource="http://www.w3.org/2001/XMLSchema#string"/>
  </owl:DatatypeProperty>
  <owl:DatatypeProperty rdf:about="http://example.org/onto/prop/yandex_mdb_postgresql_cluster_zone">
    <rdfs:label>zone</rdfs:label>
    <rdfs:comment>The [availability zone](https://yandex.cloud/docs/overview/concepts/geo-scope) where resource is located. If it is not provided, the default provider zone will be used.</rdfs:comment>
    <rdfs:domain rdf:resource="http://example.org/onto/class/yandex_mdb_postgresql_cluster"/>
    <rdfs:range rdf:resource="http://www.w3.org/2001/XMLSchema#string"/>
  </owl:DatatypeProperty>
  <owl:DatatypeProperty rdf:about="http://example.org/onto/prop/yandex_mdb_postgresql_cluster_day">
    <rdfs:label>day</rdfs:label>
    <rdfs:comment>Day of the week (in `DDD` format). Allowed values: `MON`, `TUE`, `WED`, `THU`, `FRI`, `SAT`, `SUN`</rdfs:comment>
    <rdfs:domain rdf:resource="http://example.org/onto/class/yandex_mdb_postgresql_cluster"/>
    <rdfs:range rdf:resource="http://www.w3.org/2001/XMLSchema#string"/>
  </owl:DatatypeProperty>
  <owl:DatatypeProperty rdf:about="http://example.org/onto/prop/yandex_mdb_postgresql_cluster_hour">
    <rdfs:label>hour</rdfs:label>
    <rdfs:comment>Hour of the day in UTC (in `HH` format). Allowed value is between 1 and 24.</rdfs:comment>
    <rdfs:domain rdf:resource="http://example.org/onto/class/yandex_mdb_postgresql_cluster"/>
    <rdfs:range rdf:resource="http://www.w3.org/2001/XMLSchema#string"/>
  </owl:DatatypeProperty>
  <owl:DatatypeProperty rdf:about="http://example.org/onto/prop/yandex_mdb_postgresql_cluster_type">
    <rdfs:label>type</rdfs:label>
    <rdfs:comment>Type of maintenance window. Can be either `ANYTIME` or `WEEKLY`. A day and hour of window need to be specified with weekly window.</rdfs:comment>
    <rdfs:domain rdf:resource="http://example.org/onto/class/yandex_mdb_postgresql_cluster"/>
    <rdfs:range rdf:resource="http://www.w3.org/2001/XMLSchema#string"/>
  </owl:DatatypeProperty>
  <owl:DatatypeProperty rdf:about="http://example.org/onto/prop/yandex_mdb_postgresql_cluster_backup_id">
    <rdfs:label>backup_id</rdfs:label>
    <rdfs:comment>Backup ID. The cluster will be created from the specified backup. [How to get a list of PostgreSQL backups](https://yandex.cloud/docs/managed-postgresql/operations/cluster-backups).</rdfs:comment>
    <rdfs:domain rdf:resource="http://example.org/onto/class/yandex_mdb_postgresql_cluster"/>
    <rdfs:range rdf:resource="http://www.w3.org/2001/XMLSchema#string"/>
  </owl:DatatypeProperty>
  <owl:DatatypeProperty rdf:about="http://example.org/onto/prop/yandex_mdb_postgresql_cluster_time">
    <rdfs:label>time</rdfs:label>
    <rdfs:comment>Timestamp of the moment to which the PostgreSQL cluster should be restored. (Format: `2006-01-02T15:04:05` - UTC). When not set, current time is used.</rdfs:comment>
    <rdfs:domain rdf:resource="http://example.org/onto/class/yandex_mdb_postgresql_cluster"/>
    <rdfs:range rdf:resource="http://www.w3.org/2001/XMLSchema#string"/>
  </owl:DatatypeProperty>
  <owl:DatatypeProperty rdf:about="http://example.org/onto/prop/yandex_mdb_postgresql_cluster_time_inclusive">
    <rdfs:label>time_inclusive</rdfs:label>
    <rdfs:comment>Flag that indicates whether a database should be restored to the first backup point available just after the timestamp specified in the [time] field instead of just before. Possible values:
* `false` (default) — the restore point refers to the first backup moment before [time].
* `true` — the restore point refers to the first backup point after [time].</rdfs:comment>
    <rdfs:domain rdf:resource="http://example.org/onto/class/yandex_mdb_postgresql_cluster"/>
    <rdfs:range rdf:resource="http://www.w3.org/2001/XMLSchema#string"/>
  </owl:DatatypeProperty>
  <owl:DatatypeProperty rdf:about="http://example.org/onto/prop/yandex_mdb_postgresql_cluster_create">
    <rdfs:label>create</rdfs:label>
    <rdfs:domain rdf:resource="http://example.org/onto/class/yandex_mdb_postgresql_cluster"/>
    <rdfs:range rdf:resource="http://www.w3.org/2001/XMLSchema#string"/>
  </owl:DatatypeProperty>
  <owl:DatatypeProperty rdf:about="http://example.org/onto/prop/yandex_mdb_postgresql_cluster_delete">
    <rdfs:label>delete</rdfs:label>
    <rdfs:domain rdf:resource="http://example.org/onto/class/yandex_mdb_postgresql_cluster"/>
    <rdfs:range rdf:resource="http://www.w3.org/2001/XMLSchema#string"/>
  </owl:DatatypeProperty>
  <owl:DatatypeProperty rdf:about="http://example.org/onto/prop/yandex_mdb_postgresql_cluster_update">
    <rdfs:label>update</rdfs:label>
    <rdfs:domain rdf:resource="http://example.org/onto/class/yandex_mdb_postgresql_cluster"/>
    <rdfs:range rdf:resource="http://www.w3.org/2001/XMLSchema#string"/>
  </owl:DatatypeProperty>
  <owl:DatatypeProperty rdf:about="http://example.org/onto/prop/yandex_mdb_postgresql_cluster_conn_limit">
    <rdfs:label>conn_limit</rdfs:label>
    <rdfs:comment>The maximum number of connections per user. (Default 50).</rdfs:comment>
    <rdfs:domain rdf:resource="http://example.org/onto/class/yandex_mdb_postgresql_cluster"/>
    <rdfs:range rdf:resource="http://www.w3.org/2001/XMLSchema#string"/>
  </owl:DatatypeProperty>
  <owl:DatatypeProperty rdf:about="http://example.org/onto/prop/yandex_mdb_postgresql_cluster_grants">
    <rdfs:label>grants</rdfs:label>
    <rdfs:comment>List of the user's grants.</rdfs:comment>
    <rdfs:domain rdf:resource="http://example.org/onto/class/yandex_mdb_postgresql_cluster"/>
    <rdfs:range rdf:resource="http://www.w3.org/2001/XMLSchema#string"/>
  </owl:DatatypeProperty>
  <owl:DatatypeProperty rdf:about="http://example.org/onto/prop/yandex_mdb_postgresql_cluster_login">
    <rdfs:label>login</rdfs:label>
    <rdfs:comment>User's ability to login.</rdfs:comment>
    <rdfs:domain rdf:resource="http://example.org/onto/class/yandex_mdb_postgresql_cluster"/>
    <rdfs:range rdf:resource="http://www.w3.org/2001/XMLSchema#string"/>
  </owl:DatatypeProperty>
  <owl:DatatypeProperty rdf:about="http://example.org/onto/prop/yandex_mdb_postgresql_cluster_name">
    <rdfs:label>name</rdfs:label>
    <rdfs:comment>The name of the user.</rdfs:comment>
    <rdfs:domain rdf:resource="http://example.org/onto/class/yandex_mdb_postgresql_cluster"/>
    <rdfs:range rdf:resource="http://www.w3.org/2001/XMLSchema#string"/>
  </owl:DatatypeProperty>
  <owl:DatatypeProperty rdf:about="http://example.org/onto/prop/yandex_mdb_postgresql_cluster_password">
    <rdfs:label>password</rdfs:label>
    <rdfs:comment>The password of the user.</rdfs:comment>
    <rdfs:domain rdf:resource="http://example.org/onto/class/yandex_mdb_postgresql_cluster"/>
    <rdfs:range rdf:resource="http://www.w3.org/2001/XMLSchema#string"/>
  </owl:DatatypeProperty>
  <owl:DatatypeProperty rdf:about="http://example.org/onto/prop/yandex_mdb_postgresql_cluster_settings">
    <rdfs:label>settings</rdfs:label>
    <rdfs:comment>Map of user settings. [Full description](https://yandex.cloud/docs/managed-postgresql/api-ref/grpc/Cluster/create#yandex.cloud.mdb.postgresql.v1.UserSettings).

* `default_transaction_isolation` - defines the default isolation level to be set for all new SQL transactions. One of:
  - 1: `read uncommitted`
  - 2: `read committed`
  - 3: `repeatable read`
  - 4: `serializable`

* `lock_timeout` - The maximum time (in milliseconds) for any statement to wait for acquiring a lock on an table, index, row or other database object (default 0).

* `log_min_duration_statement` - This setting controls logging of the duration of statements. Default -1 disables logging of the duration of statements.

* `synchronous_commit` - This setting defines whether DBMS will commit transaction in a synchronous way. One of:
  - 1: `on`
  - 2: `off`
  - 3: `local`
  - 4: `remote write`
  - 5: `remote apply`

* `temp_file_limit` - The maximum storage space size (in kilobytes) that a single process can use to create temporary files.

* `log_statement` - This setting specifies which SQL statements should be logged (on the user level). One of:
  - 1: `none`
  - 2: `ddl`
  - 3: `mod`
  - 4: `all`

* `pool_mode` - Mode that the connection pooler is working in with specified user. One of:
  - 1: `session`
  - 2: `transaction`
  - 3: `statement`

* `prepared_statements_pooling` - This setting allows user to use prepared statements with transaction pooling. Boolean.

* `catchup_timeout` - The connection pooler setting. It determines the maximum allowed replication lag (in seconds). Pooler will reject connections to the replica with a lag above this threshold. Default value is 0, which disables this feature. Integer.

* `wal_sender_timeout` - The maximum time (in milliseconds) to wait for WAL replication. Terminate replication connections that are inactive for longer than this amount of time. Integer.

* `idle_in_transaction_session_timeout` - Sets the maximum allowed idle time (in milliseconds) between queries, when in a transaction. Value of 0 (default) disables the timeout. Integer.

* `statement_timeout` - The maximum time (in milliseconds) to wait for statement. Value of 0 (default) disables the timeout. Integer.</rdfs:comment>
    <rdfs:domain rdf:resource="http://example.org/onto/class/yandex_mdb_postgresql_cluster"/>
    <rdfs:range rdf:resource="http://www.w3.org/2001/XMLSchema#string"/>
  </owl:DatatypeProperty>
  <owl:DatatypeProperty rdf:about="http://example.org/onto/prop/yandex_mdb_postgresql_cluster_database_name">
    <rdfs:label>database_name</rdfs:label>
    <rdfs:comment>The name of the database that the permission grants access to.</rdfs:comment>
    <rdfs:domain rdf:resource="http://example.org/onto/class/yandex_mdb_postgresql_cluster"/>
    <rdfs:range rdf:resource="http://www.w3.org/2001/XMLSchema#string"/>
  </owl:DatatypeProperty>
</rdf:RDF>
