<?xml version="1.0" encoding="UTF-8"?>
<rdf:RDF
  xmlns:rdf="http://www.w3.org/1999/02/22-rdf-syntax-ns#"
  xmlns:rdfs="http://www.w3.org/2000/01/rdf-schema#"
  xmlns:owl="http://www.w3.org/2002/07/owl#"
  xmlns:xsd="http://www.w3.org/2001/XMLSchema#"
  xml:base="http://example.org/onto/">
  <owl:Class rdf:about="http://example.org/onto/class/yandex_cloudregistry_registry_ip_permission">
    <rdfs:label>yandex_cloudregistry_registry_ip_permission</rdfs:label>
    <rdfs:comment>Creates a new Cloud Registry IP Permission. For more information, see [the official documentation](https://yandex.cloud/docs/cloud-registry/operations/registry/registry-access)</rdfs:comment>
  </owl:Class>
  <owl:DatatypeProperty rdf:about="http://example.org/onto/prop/yandex_cloudregistry_registry_ip_permission_id">
    <rdfs:label>id</rdfs:label>
    <rdfs:comment>The ID of IP permission.</rdfs:comment>
    <rdfs:domain rdf:resource="http://example.org/onto/class/yandex_cloudregistry_registry_ip_permission"/>
    <rdfs:range rdf:resource="http://www.w3.org/2001/XMLSchema#string"/>
  </owl:DatatypeProperty>
  <owl:DatatypeProperty rdf:about="http://example.org/onto/prop/yandex_cloudregistry_registry_ip_permission_pull">
    <rdfs:label>pull</rdfs:label>
    <rdfs:comment>List of configured CIDRs from which `pull` operations are allowed.</rdfs:comment>
    <rdfs:domain rdf:resource="http://example.org/onto/class/yandex_cloudregistry_registry_ip_permission"/>
    <rdfs:range rdf:resource="http://www.w3.org/2001/XMLSchema#string"/>
  </owl:DatatypeProperty>
  <owl:DatatypeProperty rdf:about="http://example.org/onto/prop/yandex_cloudregistry_registry_ip_permission_push">
    <rdfs:label>push</rdfs:label>
    <rdfs:comment>List of configured CIDRs from which `push` operations are allowed.</rdfs:comment>
    <rdfs:domain rdf:resource="http://example.org/onto/class/yandex_cloudregistry_registry_ip_permission"/>
    <rdfs:range rdf:resource="http://www.w3.org/2001/XMLSchema#string"/>
  </owl:DatatypeProperty>
  <owl:DatatypeProperty rdf:about="http://example.org/onto/prop/yandex_cloudregistry_registry_ip_permission_registry_id">
    <rdfs:label>registry_id</rdfs:label>
    <rdfs:comment>The ID of the registry that IP restrictions are applied to.</rdfs:comment>
    <rdfs:domain rdf:resource="http://example.org/onto/class/yandex_cloudregistry_registry_ip_permission"/>
    <rdfs:range rdf:resource="http://www.w3.org/2001/XMLSchema#string"/>
  </owl:DatatypeProperty>
  <owl:DatatypeProperty rdf:about="http://example.org/onto/prop/yandex_cloudregistry_registry_ip_permission_timeouts">
    <rdfs:label>timeouts</rdfs:label>
    <rdfs:domain rdf:resource="http://example.org/onto/class/yandex_cloudregistry_registry_ip_permission"/>
    <rdfs:range rdf:resource="http://www.w3.org/2001/XMLSchema#string"/>
  </owl:DatatypeProperty>
</rdf:RDF>
