<?xml version="1.0" encoding="UTF-8"?>
<rdf:RDF
  xmlns:rdf="http://www.w3.org/1999/02/22-rdf-syntax-ns#"
  xmlns:rdfs="http://www.w3.org/2000/01/rdf-schema#"
  xmlns:owl="http://www.w3.org/2002/07/owl#"
  xmlns:xsd="http://www.w3.org/2001/XMLSchema#"
  xml:base="http://example.org/onto/">
  <owl:Class rdf:about="http://example.org/onto/class/yandex_iam_service_account_key">
    <rdfs:label>yandex_iam_service_account_key</rdfs:label>
    <rdfs:comment>Allows management of [Yandex Cloud IAM service account authorized keys](https://yandex.cloud/docs/iam/concepts/authorization/key). Generated pair of keys is used to create a [JSON Web Token](https://tools.ietf.org/html/rfc7519) which is necessary for requesting an [IAM Token](https://yandex.cloud/docs/iam/concepts/authorization/iam-token) for a [service account](https://yandex.cloud/docs/iam/concepts/users/service-accounts).</rdfs:comment>
  </owl:Class>
  <owl:DatatypeProperty rdf:about="http://example.org/onto/prop/yandex_iam_service_account_key_created_at">
    <rdfs:label>created_at</rdfs:label>
    <rdfs:comment>The creation timestamp of the resource.</rdfs:comment>
    <rdfs:domain rdf:resource="http://example.org/onto/class/yandex_iam_service_account_key"/>
    <rdfs:range rdf:resource="http://www.w3.org/2001/XMLSchema#string"/>
  </owl:DatatypeProperty>
  <owl:DatatypeProperty rdf:about="http://example.org/onto/prop/yandex_iam_service_account_key_description">
    <rdfs:label>description</rdfs:label>
    <rdfs:comment>The resource description.</rdfs:comment>
    <rdfs:domain rdf:resource="http://example.org/onto/class/yandex_iam_service_account_key"/>
    <rdfs:range rdf:resource="http://www.w3.org/2001/XMLSchema#string"/>
  </owl:DatatypeProperty>
  <owl:DatatypeProperty rdf:about="http://example.org/onto/prop/yandex_iam_service_account_key_encrypted_private_key">
    <rdfs:label>encrypted_private_key</rdfs:label>
    <rdfs:comment>The encrypted private key, base64 encoded. This is only populated when `pgp_key` is supplied.</rdfs:comment>
    <rdfs:domain rdf:resource="http://example.org/onto/class/yandex_iam_service_account_key"/>
    <rdfs:range rdf:resource="http://www.w3.org/2001/XMLSchema#string"/>
  </owl:DatatypeProperty>
  <owl:DatatypeProperty rdf:about="http://example.org/onto/prop/yandex_iam_service_account_key_format">
    <rdfs:label>format</rdfs:label>
    <rdfs:comment>The output format of the keys. `PEM_FILE` is the default format.</rdfs:comment>
    <rdfs:domain rdf:resource="http://example.org/onto/class/yandex_iam_service_account_key"/>
    <rdfs:range rdf:resource="http://www.w3.org/2001/XMLSchema#string"/>
  </owl:DatatypeProperty>
  <owl:DatatypeProperty rdf:about="http://example.org/onto/prop/yandex_iam_service_account_key_id">
    <rdfs:label>id</rdfs:label>
    <rdfs:domain rdf:resource="http://example.org/onto/class/yandex_iam_service_account_key"/>
    <rdfs:range rdf:resource="http://www.w3.org/2001/XMLSchema#string"/>
  </owl:DatatypeProperty>
  <owl:DatatypeProperty rdf:about="http://example.org/onto/prop/yandex_iam_service_account_key_key_algorithm">
    <rdfs:label>key_algorithm</rdfs:label>
    <rdfs:comment>The algorithm used to generate the key. `RSA_2048` is the default algorithm. Valid values are listed in the [API reference](https://yandex.cloud/docs/iam/api-ref/Key).</rdfs:comment>
    <rdfs:domain rdf:resource="http://example.org/onto/class/yandex_iam_service_account_key"/>
    <rdfs:range rdf:resource="http://www.w3.org/2001/XMLSchema#string"/>
  </owl:DatatypeProperty>
  <owl:DatatypeProperty rdf:about="http://example.org/onto/prop/yandex_iam_service_account_key_key_fingerprint">
    <rdfs:label>key_fingerprint</rdfs:label>
    <rdfs:comment>The fingerprint of the PGP key used to encrypt the private key. This is only populated when `pgp_key` is supplied.</rdfs:comment>
    <rdfs:domain rdf:resource="http://example.org/onto/class/yandex_iam_service_account_key"/>
    <rdfs:range rdf:resource="http://www.w3.org/2001/XMLSchema#string"/>
  </owl:DatatypeProperty>
  <owl:DatatypeProperty rdf:about="http://example.org/onto/prop/yandex_iam_service_account_key_output_to_lockbox_version_id">
    <rdfs:label>output_to_lockbox_version_id</rdfs:label>
    <rdfs:comment>ID of the Lockbox secret version that contains the value of `secret_key`. This is only populated when `output_to_lockbox` is supplied. This version will be destroyed when the IAM key is destroyed, or when `output_to_lockbox` is removed.</rdfs:comment>
    <rdfs:domain rdf:resource="http://example.org/onto/class/yandex_iam_service_account_key"/>
    <rdfs:range rdf:resource="http://www.w3.org/2001/XMLSchema#string"/>
  </owl:DatatypeProperty>
  <owl:DatatypeProperty rdf:about="http://example.org/onto/prop/yandex_iam_service_account_key_pgp_key">
    <rdfs:label>pgp_key</rdfs:label>
    <rdfs:comment>An optional PGP key to encrypt the resulting private key material. May either be a base64-encoded public key or a keybase username in the form `keybase:keybaseusername`.</rdfs:comment>
    <rdfs:domain rdf:resource="http://example.org/onto/class/yandex_iam_service_account_key"/>
    <rdfs:range rdf:resource="http://www.w3.org/2001/XMLSchema#string"/>
  </owl:DatatypeProperty>
  <owl:DatatypeProperty rdf:about="http://example.org/onto/prop/yandex_iam_service_account_key_private_key">
    <rdfs:label>private_key</rdfs:label>
    <rdfs:comment>The private key. This is only populated when neither `pgp_key` nor `output_to_lockbox` are provided.</rdfs:comment>
    <rdfs:domain rdf:resource="http://example.org/onto/class/yandex_iam_service_account_key"/>
    <rdfs:range rdf:resource="http://www.w3.org/2001/XMLSchema#string"/>
  </owl:DatatypeProperty>
  <owl:DatatypeProperty rdf:about="http://example.org/onto/prop/yandex_iam_service_account_key_public_key">
    <rdfs:label>public_key</rdfs:label>
    <rdfs:comment>The public key.</rdfs:comment>
    <rdfs:domain rdf:resource="http://example.org/onto/class/yandex_iam_service_account_key"/>
    <rdfs:range rdf:resource="http://www.w3.org/2001/XMLSchema#string"/>
  </owl:DatatypeProperty>
  <owl:DatatypeProperty rdf:about="http://example.org/onto/prop/yandex_iam_service_account_key_service_account_id">
    <rdfs:label>service_account_id</rdfs:label>
    <rdfs:comment>ID of the service account to create a pair for.</rdfs:comment>
    <rdfs:domain rdf:resource="http://example.org/onto/class/yandex_iam_service_account_key"/>
    <rdfs:range rdf:resource="http://www.w3.org/2001/XMLSchema#string"/>
  </owl:DatatypeProperty>
  <owl:DatatypeProperty rdf:about="http://example.org/onto/prop/yandex_iam_service_account_key_entry_for_private_key">
    <rdfs:label>entry_for_private_key</rdfs:label>
    <rdfs:comment>entry that will store the value of private_key</rdfs:comment>
    <rdfs:domain rdf:resource="http://example.org/onto/class/yandex_iam_service_account_key"/>
    <rdfs:range rdf:resource="http://www.w3.org/2001/XMLSchema#string"/>
  </owl:DatatypeProperty>
  <owl:DatatypeProperty rdf:about="http://example.org/onto/prop/yandex_iam_service_account_key_secret_id">
    <rdfs:label>secret_id</rdfs:label>
    <rdfs:comment>ID of the Lockbox secret where to store the sensible values.</rdfs:comment>
    <rdfs:domain rdf:resource="http://example.org/onto/class/yandex_iam_service_account_key"/>
    <rdfs:range rdf:resource="http://www.w3.org/2001/XMLSchema#string"/>
  </owl:DatatypeProperty>
</rdf:RDF>
