<?xml version="1.0" encoding="UTF-8"?>
<rdf:RDF
  xmlns:rdf="http://www.w3.org/1999/02/22-rdf-syntax-ns#"
  xmlns:rdfs="http://www.w3.org/2000/01/rdf-schema#"
  xmlns:owl="http://www.w3.org/2002/07/owl#"
  xmlns:xsd="http://www.w3.org/2001/XMLSchema#"
  xml:base="http://example.org/onto/">
  <owl:Class rdf:about="http://example.org/onto/class/yandex_storage_bucket">
    <rdfs:label>yandex_storage_bucket</rdfs:label>
    <rdfs:comment>Allows management of [Yandex Cloud Storage Bucket](https://yandex.cloud/docs/storage/concepts/bucket).

~> By default, for authentication, you need to use [IAM token](https://yandex.cloud/docs/iam/concepts/authorization/iam-token) with the necessary permissions.

~> Alternatively, you can provide [static access keys](https://yandex.cloud/docs/iam/concepts/authorization/access-key) (Access and Secret). To generate these keys, you will need a Service Account with the appropriate permissions.

~> For extended API usage, such as setting the `max_size`, `folder_id`, `anonymous_access_flags`, `default_storage_class`, and `https` parameters for a bucket, only the default authorization method will be used. This means the `IAM` token from the `provider` block will be applied.
This can be confusing in cases where a separate service account is used for managing buckets because, in such scenarios,buckets may be accessed by two different accounts, each with potentially different permissions for the buckets.

~> In case you are using IAM token from UserAccount, you are needed to explicitly specify `folder_id` in the resource, as it cannot be identified from such type of account. In case you are using IAM token from ServiceAccount or static access keys, `folder_id` does not need to be specified unless you want to create the resource in a different folder than the account folder.

~> Terraform will import this resource with `force_destroy` set to `false` in state. If you've set it to `true` in config, run `terraform apply` to update the value set in state. If you delete this resource before updating the value, objects in the bucket will not be destroyed.</rdfs:comment>
  </owl:Class>
  <owl:DatatypeProperty rdf:about="http://example.org/onto/prop/yandex_storage_bucket_access_key">
    <rdfs:label>access_key</rdfs:label>
    <rdfs:comment>The access key to use when applying changes. This value can also be provided as `storage_access_key` specified in provider config (explicitly or within `shared_credentials_file`) is used.</rdfs:comment>
    <rdfs:domain rdf:resource="http://example.org/onto/class/yandex_storage_bucket"/>
    <rdfs:range rdf:resource="http://www.w3.org/2001/XMLSchema#string"/>
  </owl:DatatypeProperty>
  <owl:DatatypeProperty rdf:about="http://example.org/onto/prop/yandex_storage_bucket_acl">
    <rdfs:label>acl</rdfs:label>
    <rdfs:comment>The [predefined ACL](https://yandex.cloud/docs/storage/concepts/acl#predefined_acls) to apply. Defaults to `private`. Conflicts with `grant`.

~> To change ACL after creation, service account with `storage.admin` role should be used, though this role is not necessary to create a bucket with any ACL.</rdfs:comment>
    <rdfs:domain rdf:resource="http://example.org/onto/class/yandex_storage_bucket"/>
    <rdfs:range rdf:resource="http://www.w3.org/2001/XMLSchema#string"/>
  </owl:DatatypeProperty>
  <owl:DatatypeProperty rdf:about="http://example.org/onto/prop/yandex_storage_bucket_bucket">
    <rdfs:label>bucket</rdfs:label>
    <rdfs:comment>The name of the bucket. If omitted, Terraform will assign a random, unique name.</rdfs:comment>
    <rdfs:domain rdf:resource="http://example.org/onto/class/yandex_storage_bucket"/>
    <rdfs:range rdf:resource="http://www.w3.org/2001/XMLSchema#string"/>
  </owl:DatatypeProperty>
  <owl:DatatypeProperty rdf:about="http://example.org/onto/prop/yandex_storage_bucket_bucket_domain_name">
    <rdfs:label>bucket_domain_name</rdfs:label>
    <rdfs:comment>The bucket domain name.</rdfs:comment>
    <rdfs:domain rdf:resource="http://example.org/onto/class/yandex_storage_bucket"/>
    <rdfs:range rdf:resource="http://www.w3.org/2001/XMLSchema#string"/>
  </owl:DatatypeProperty>
  <owl:DatatypeProperty rdf:about="http://example.org/onto/prop/yandex_storage_bucket_bucket_prefix">
    <rdfs:label>bucket_prefix</rdfs:label>
    <rdfs:comment>Creates a unique bucket name beginning with the specified prefix. Conflicts with `bucket`.</rdfs:comment>
    <rdfs:domain rdf:resource="http://example.org/onto/class/yandex_storage_bucket"/>
    <rdfs:range rdf:resource="http://www.w3.org/2001/XMLSchema#string"/>
  </owl:DatatypeProperty>
  <owl:DatatypeProperty rdf:about="http://example.org/onto/prop/yandex_storage_bucket_default_storage_class">
    <rdfs:label>default_storage_class</rdfs:label>
    <rdfs:comment>Storage class which is used for storing objects by default. Available values are: "STANDARD", "COLD", "ICE". Default is `"STANDARD"`. See [Storage Class](https://yandex.cloud/docs/storage/concepts/storage-class) for more information.</rdfs:comment>
    <rdfs:domain rdf:resource="http://example.org/onto/class/yandex_storage_bucket"/>
    <rdfs:range rdf:resource="http://www.w3.org/2001/XMLSchema#string"/>
  </owl:DatatypeProperty>
  <owl:DatatypeProperty rdf:about="http://example.org/onto/prop/yandex_storage_bucket_folder_id">
    <rdfs:label>folder_id</rdfs:label>
    <rdfs:comment>Allow to create bucket in different folder. In case you are using IAM token from UserAccount, you are needed to explicitly specify folder_id in the resource, as it cannot be identified from such type of account. In case you are using IAM token from ServiceAccount or static access keys, folder_id does not need to be specified unless you want to create the resource in a different folder than the account folder.

~> It will try to create bucket using `IAM-token`, not using `access keys`.</rdfs:comment>
    <rdfs:domain rdf:resource="http://example.org/onto/class/yandex_storage_bucket"/>
    <rdfs:range rdf:resource="http://www.w3.org/2001/XMLSchema#string"/>
  </owl:DatatypeProperty>
  <owl:DatatypeProperty rdf:about="http://example.org/onto/prop/yandex_storage_bucket_force_destroy">
    <rdfs:label>force_destroy</rdfs:label>
    <rdfs:comment>A boolean that indicates all objects should be deleted from the bucket so that the bucket can be destroyed without error. These objects are *not* recoverable. Default is `false`.</rdfs:comment>
    <rdfs:domain rdf:resource="http://example.org/onto/class/yandex_storage_bucket"/>
    <rdfs:range rdf:resource="http://www.w3.org/2001/XMLSchema#string"/>
  </owl:DatatypeProperty>
  <owl:DatatypeProperty rdf:about="http://example.org/onto/prop/yandex_storage_bucket_id">
    <rdfs:label>id</rdfs:label>
    <rdfs:domain rdf:resource="http://example.org/onto/class/yandex_storage_bucket"/>
    <rdfs:range rdf:resource="http://www.w3.org/2001/XMLSchema#string"/>
  </owl:DatatypeProperty>
  <owl:DatatypeProperty rdf:about="http://example.org/onto/prop/yandex_storage_bucket_max_size">
    <rdfs:label>max_size</rdfs:label>
    <rdfs:comment>The size of bucket, in bytes. See [Size Limiting](https://yandex.cloud/docs/storage/operations/buckets/limit-max-volume) for more information.</rdfs:comment>
    <rdfs:domain rdf:resource="http://example.org/onto/class/yandex_storage_bucket"/>
    <rdfs:range rdf:resource="http://www.w3.org/2001/XMLSchema#string"/>
  </owl:DatatypeProperty>
  <owl:DatatypeProperty rdf:about="http://example.org/onto/prop/yandex_storage_bucket_policy">
    <rdfs:label>policy</rdfs:label>
    <rdfs:comment>The `policy` object should contain the only field with the text of the policy. See [policy documentation](https://yandex.cloud/docs/storage/concepts/policy) for more information on policy format.</rdfs:comment>
    <rdfs:domain rdf:resource="http://example.org/onto/class/yandex_storage_bucket"/>
    <rdfs:range rdf:resource="http://www.w3.org/2001/XMLSchema#string"/>
  </owl:DatatypeProperty>
  <owl:DatatypeProperty rdf:about="http://example.org/onto/prop/yandex_storage_bucket_secret_key">
    <rdfs:label>secret_key</rdfs:label>
    <rdfs:comment>The secret key to use when applying changes. This value can also be provided as `storage_secret_key` specified in provider config (explicitly or within `shared_credentials_file`) is used.</rdfs:comment>
    <rdfs:domain rdf:resource="http://example.org/onto/class/yandex_storage_bucket"/>
    <rdfs:range rdf:resource="http://www.w3.org/2001/XMLSchema#string"/>
  </owl:DatatypeProperty>
  <owl:DatatypeProperty rdf:about="http://example.org/onto/prop/yandex_storage_bucket_tags">
    <rdfs:label>tags</rdfs:label>
    <rdfs:comment>The `tags` object for setting tags (or labels) for bucket. See [Tags](https://yandex.cloud/docs/storage/concepts/tags) for more information.</rdfs:comment>
    <rdfs:domain rdf:resource="http://example.org/onto/class/yandex_storage_bucket"/>
    <rdfs:range rdf:resource="http://www.w3.org/2001/XMLSchema#string"/>
  </owl:DatatypeProperty>
  <owl:DatatypeProperty rdf:about="http://example.org/onto/prop/yandex_storage_bucket_website_domain">
    <rdfs:label>website_domain</rdfs:label>
    <rdfs:comment>The domain of the website endpoint, if the bucket is configured with a website. If not, this will be an empty string.</rdfs:comment>
    <rdfs:domain rdf:resource="http://example.org/onto/class/yandex_storage_bucket"/>
    <rdfs:range rdf:resource="http://www.w3.org/2001/XMLSchema#string"/>
  </owl:DatatypeProperty>
  <owl:DatatypeProperty rdf:about="http://example.org/onto/prop/yandex_storage_bucket_website_endpoint">
    <rdfs:label>website_endpoint</rdfs:label>
    <rdfs:comment>The website endpoint, if the bucket is configured with a website. If not, this will be an empty string.</rdfs:comment>
    <rdfs:domain rdf:resource="http://example.org/onto/class/yandex_storage_bucket"/>
    <rdfs:range rdf:resource="http://www.w3.org/2001/XMLSchema#string"/>
  </owl:DatatypeProperty>
  <owl:DatatypeProperty rdf:about="http://example.org/onto/prop/yandex_storage_bucket_config_read">
    <rdfs:label>config_read</rdfs:label>
    <rdfs:comment>Allows to read bucket configuration anonymously.</rdfs:comment>
    <rdfs:domain rdf:resource="http://example.org/onto/class/yandex_storage_bucket"/>
    <rdfs:range rdf:resource="http://www.w3.org/2001/XMLSchema#string"/>
  </owl:DatatypeProperty>
  <owl:DatatypeProperty rdf:about="http://example.org/onto/prop/yandex_storage_bucket_list">
    <rdfs:label>list</rdfs:label>
    <rdfs:comment>Allows to list object in bucket anonymously.</rdfs:comment>
    <rdfs:domain rdf:resource="http://example.org/onto/class/yandex_storage_bucket"/>
    <rdfs:range rdf:resource="http://www.w3.org/2001/XMLSchema#string"/>
  </owl:DatatypeProperty>
  <owl:DatatypeProperty rdf:about="http://example.org/onto/prop/yandex_storage_bucket_read">
    <rdfs:label>read</rdfs:label>
    <rdfs:comment>Allows to read objects in bucket anonymously.</rdfs:comment>
    <rdfs:domain rdf:resource="http://example.org/onto/class/yandex_storage_bucket"/>
    <rdfs:range rdf:resource="http://www.w3.org/2001/XMLSchema#string"/>
  </owl:DatatypeProperty>
  <owl:DatatypeProperty rdf:about="http://example.org/onto/prop/yandex_storage_bucket_allowed_headers">
    <rdfs:label>allowed_headers</rdfs:label>
    <rdfs:comment>Specifies which headers are allowed.</rdfs:comment>
    <rdfs:domain rdf:resource="http://example.org/onto/class/yandex_storage_bucket"/>
    <rdfs:range rdf:resource="http://www.w3.org/2001/XMLSchema#string"/>
  </owl:DatatypeProperty>
  <owl:DatatypeProperty rdf:about="http://example.org/onto/prop/yandex_storage_bucket_allowed_methods">
    <rdfs:label>allowed_methods</rdfs:label>
    <rdfs:comment>Specifies which methods are allowed. Can be `GET`, `PUT`, `POST`, `DELETE` or `HEAD`.</rdfs:comment>
    <rdfs:domain rdf:resource="http://example.org/onto/class/yandex_storage_bucket"/>
    <rdfs:range rdf:resource="http://www.w3.org/2001/XMLSchema#string"/>
  </owl:DatatypeProperty>
  <owl:DatatypeProperty rdf:about="http://example.org/onto/prop/yandex_storage_bucket_allowed_origins">
    <rdfs:label>allowed_origins</rdfs:label>
    <rdfs:comment>Specifies which origins are allowed.</rdfs:comment>
    <rdfs:domain rdf:resource="http://example.org/onto/class/yandex_storage_bucket"/>
    <rdfs:range rdf:resource="http://www.w3.org/2001/XMLSchema#string"/>
  </owl:DatatypeProperty>
  <owl:DatatypeProperty rdf:about="http://example.org/onto/prop/yandex_storage_bucket_expose_headers">
    <rdfs:label>expose_headers</rdfs:label>
    <rdfs:comment>Specifies expose header in the response.</rdfs:comment>
    <rdfs:domain rdf:resource="http://example.org/onto/class/yandex_storage_bucket"/>
    <rdfs:range rdf:resource="http://www.w3.org/2001/XMLSchema#string"/>
  </owl:DatatypeProperty>
  <owl:DatatypeProperty rdf:about="http://example.org/onto/prop/yandex_storage_bucket_max_age_seconds">
    <rdfs:label>max_age_seconds</rdfs:label>
    <rdfs:comment>Specifies time in seconds that browser can cache the response for a preflight request.</rdfs:comment>
    <rdfs:domain rdf:resource="http://example.org/onto/class/yandex_storage_bucket"/>
    <rdfs:range rdf:resource="http://www.w3.org/2001/XMLSchema#string"/>
  </owl:DatatypeProperty>
  <owl:DatatypeProperty rdf:about="http://example.org/onto/prop/yandex_storage_bucket_id">
    <rdfs:label>id</rdfs:label>
    <rdfs:comment>Canonical user id to grant for. Used only when type is `CanonicalUser`.</rdfs:comment>
    <rdfs:domain rdf:resource="http://example.org/onto/class/yandex_storage_bucket"/>
    <rdfs:range rdf:resource="http://www.w3.org/2001/XMLSchema#string"/>
  </owl:DatatypeProperty>
  <owl:DatatypeProperty rdf:about="http://example.org/onto/prop/yandex_storage_bucket_permissions">
    <rdfs:label>permissions</rdfs:label>
    <rdfs:comment>List of permissions to apply for grantee. Valid values are `READ`, `WRITE`, `FULL_CONTROL`.</rdfs:comment>
    <rdfs:domain rdf:resource="http://example.org/onto/class/yandex_storage_bucket"/>
    <rdfs:range rdf:resource="http://www.w3.org/2001/XMLSchema#string"/>
  </owl:DatatypeProperty>
  <owl:DatatypeProperty rdf:about="http://example.org/onto/prop/yandex_storage_bucket_type">
    <rdfs:label>type</rdfs:label>
    <rdfs:comment>Type of grantee to apply for. Valid values are `CanonicalUser` and `Group`.</rdfs:comment>
    <rdfs:domain rdf:resource="http://example.org/onto/class/yandex_storage_bucket"/>
    <rdfs:range rdf:resource="http://www.w3.org/2001/XMLSchema#string"/>
  </owl:DatatypeProperty>
  <owl:DatatypeProperty rdf:about="http://example.org/onto/prop/yandex_storage_bucket_uri">
    <rdfs:label>uri</rdfs:label>
    <rdfs:comment>URI address to grant for. Used only when type is Group.</rdfs:comment>
    <rdfs:domain rdf:resource="http://example.org/onto/class/yandex_storage_bucket"/>
    <rdfs:range rdf:resource="http://www.w3.org/2001/XMLSchema#string"/>
  </owl:DatatypeProperty>
  <owl:DatatypeProperty rdf:about="http://example.org/onto/prop/yandex_storage_bucket_certificate_id">
    <rdfs:label>certificate_id</rdfs:label>
    <rdfs:comment>Id of the certificate in Certificate Manager, that will be used for bucket.</rdfs:comment>
    <rdfs:domain rdf:resource="http://example.org/onto/class/yandex_storage_bucket"/>
    <rdfs:range rdf:resource="http://www.w3.org/2001/XMLSchema#string"/>
  </owl:DatatypeProperty>
  <owl:DatatypeProperty rdf:about="http://example.org/onto/prop/yandex_storage_bucket_abort_incomplete_multipart_upload_days">
    <rdfs:label>abort_incomplete_multipart_upload_days</rdfs:label>
    <rdfs:comment>Specifies the number of days after initiating a multipart upload when the multipart upload must be completed.</rdfs:comment>
    <rdfs:domain rdf:resource="http://example.org/onto/class/yandex_storage_bucket"/>
    <rdfs:range rdf:resource="http://www.w3.org/2001/XMLSchema#string"/>
  </owl:DatatypeProperty>
  <owl:DatatypeProperty rdf:about="http://example.org/onto/prop/yandex_storage_bucket_enabled">
    <rdfs:label>enabled</rdfs:label>
    <rdfs:comment>Specifies lifecycle rule status.</rdfs:comment>
    <rdfs:domain rdf:resource="http://example.org/onto/class/yandex_storage_bucket"/>
    <rdfs:range rdf:resource="http://www.w3.org/2001/XMLSchema#string"/>
  </owl:DatatypeProperty>
  <owl:DatatypeProperty rdf:about="http://example.org/onto/prop/yandex_storage_bucket_id">
    <rdfs:label>id</rdfs:label>
    <rdfs:comment>Unique identifier for the rule. Must be less than or equal to 255 characters in length.</rdfs:comment>
    <rdfs:domain rdf:resource="http://example.org/onto/class/yandex_storage_bucket"/>
    <rdfs:range rdf:resource="http://www.w3.org/2001/XMLSchema#string"/>
  </owl:DatatypeProperty>
  <owl:DatatypeProperty rdf:about="http://example.org/onto/prop/yandex_storage_bucket_prefix">
    <rdfs:label>prefix</rdfs:label>
    <rdfs:comment>Object key prefix identifying one or more objects to which the rule applies.</rdfs:comment>
    <rdfs:domain rdf:resource="http://example.org/onto/class/yandex_storage_bucket"/>
    <rdfs:range rdf:resource="http://www.w3.org/2001/XMLSchema#string"/>
  </owl:DatatypeProperty>
  <owl:DatatypeProperty rdf:about="http://example.org/onto/prop/yandex_storage_bucket_date">
    <rdfs:label>date</rdfs:label>
    <rdfs:comment>Specifies the date after which you want the corresponding action to take effect.</rdfs:comment>
    <rdfs:domain rdf:resource="http://example.org/onto/class/yandex_storage_bucket"/>
    <rdfs:range rdf:resource="http://www.w3.org/2001/XMLSchema#string"/>
  </owl:DatatypeProperty>
  <owl:DatatypeProperty rdf:about="http://example.org/onto/prop/yandex_storage_bucket_days">
    <rdfs:label>days</rdfs:label>
    <rdfs:comment>Specifies the number of days after object creation when the specific rule action takes effect.</rdfs:comment>
    <rdfs:domain rdf:resource="http://example.org/onto/class/yandex_storage_bucket"/>
    <rdfs:range rdf:resource="http://www.w3.org/2001/XMLSchema#string"/>
  </owl:DatatypeProperty>
  <owl:DatatypeProperty rdf:about="http://example.org/onto/prop/yandex_storage_bucket_expired_object_delete_marker">
    <rdfs:label>expired_object_delete_marker</rdfs:label>
    <rdfs:comment>n a versioned bucket (versioning-enabled or versioning-suspended bucket), you can add this element in the lifecycle configuration to direct Object Storage to delete expired object delete markers.</rdfs:comment>
    <rdfs:domain rdf:resource="http://example.org/onto/class/yandex_storage_bucket"/>
    <rdfs:range rdf:resource="http://www.w3.org/2001/XMLSchema#string"/>
  </owl:DatatypeProperty>
  <owl:DatatypeProperty rdf:about="http://example.org/onto/prop/yandex_storage_bucket_object_size_greater_than">
    <rdfs:label>object_size_greater_than</rdfs:label>
    <rdfs:comment>Minimum object size to which the rule applies.</rdfs:comment>
    <rdfs:domain rdf:resource="http://example.org/onto/class/yandex_storage_bucket"/>
    <rdfs:range rdf:resource="http://www.w3.org/2001/XMLSchema#string"/>
  </owl:DatatypeProperty>
  <owl:DatatypeProperty rdf:about="http://example.org/onto/prop/yandex_storage_bucket_object_size_less_than">
    <rdfs:label>object_size_less_than</rdfs:label>
    <rdfs:comment>Maximum object size to which the rule applies.</rdfs:comment>
    <rdfs:domain rdf:resource="http://example.org/onto/class/yandex_storage_bucket"/>
    <rdfs:range rdf:resource="http://www.w3.org/2001/XMLSchema#string"/>
  </owl:DatatypeProperty>
  <owl:DatatypeProperty rdf:about="http://example.org/onto/prop/yandex_storage_bucket_prefix">
    <rdfs:label>prefix</rdfs:label>
    <rdfs:comment>Object key prefix identifying one or more objects to which the rule applies.</rdfs:comment>
    <rdfs:domain rdf:resource="http://example.org/onto/class/yandex_storage_bucket"/>
    <rdfs:range rdf:resource="http://www.w3.org/2001/XMLSchema#string"/>
  </owl:DatatypeProperty>
  <owl:DatatypeProperty rdf:about="http://example.org/onto/prop/yandex_storage_bucket_object_size_greater_than">
    <rdfs:label>object_size_greater_than</rdfs:label>
    <rdfs:comment>Minimum object size to which the rule applies.</rdfs:comment>
    <rdfs:domain rdf:resource="http://example.org/onto/class/yandex_storage_bucket"/>
    <rdfs:range rdf:resource="http://www.w3.org/2001/XMLSchema#string"/>
  </owl:DatatypeProperty>
  <owl:DatatypeProperty rdf:about="http://example.org/onto/prop/yandex_storage_bucket_object_size_less_than">
    <rdfs:label>object_size_less_than</rdfs:label>
    <rdfs:comment>Maximum object size to which the rule applies.</rdfs:comment>
    <rdfs:domain rdf:resource="http://example.org/onto/class/yandex_storage_bucket"/>
    <rdfs:range rdf:resource="http://www.w3.org/2001/XMLSchema#string"/>
  </owl:DatatypeProperty>
  <owl:DatatypeProperty rdf:about="http://example.org/onto/prop/yandex_storage_bucket_prefix">
    <rdfs:label>prefix</rdfs:label>
    <rdfs:comment>Object key prefix identifying one or more objects to which the rule applies.</rdfs:comment>
    <rdfs:domain rdf:resource="http://example.org/onto/class/yandex_storage_bucket"/>
    <rdfs:range rdf:resource="http://www.w3.org/2001/XMLSchema#string"/>
  </owl:DatatypeProperty>
  <owl:DatatypeProperty rdf:about="http://example.org/onto/prop/yandex_storage_bucket_tags">
    <rdfs:label>tags</rdfs:label>
    <rdfs:comment>The `tags` object for setting tags (or labels) for bucket. See [Tags](https://yandex.cloud/docs/storage/concepts/tags) for more information.</rdfs:comment>
    <rdfs:domain rdf:resource="http://example.org/onto/class/yandex_storage_bucket"/>
    <rdfs:range rdf:resource="http://www.w3.org/2001/XMLSchema#string"/>
  </owl:DatatypeProperty>
  <owl:DatatypeProperty rdf:about="http://example.org/onto/prop/yandex_storage_bucket_key">
    <rdfs:label>key</rdfs:label>
    <rdfs:comment>A key.</rdfs:comment>
    <rdfs:domain rdf:resource="http://example.org/onto/class/yandex_storage_bucket"/>
    <rdfs:range rdf:resource="http://www.w3.org/2001/XMLSchema#string"/>
  </owl:DatatypeProperty>
  <owl:DatatypeProperty rdf:about="http://example.org/onto/prop/yandex_storage_bucket_value">
    <rdfs:label>value</rdfs:label>
    <rdfs:comment>A value.</rdfs:comment>
    <rdfs:domain rdf:resource="http://example.org/onto/class/yandex_storage_bucket"/>
    <rdfs:range rdf:resource="http://www.w3.org/2001/XMLSchema#string"/>
  </owl:DatatypeProperty>
  <owl:DatatypeProperty rdf:about="http://example.org/onto/prop/yandex_storage_bucket_days">
    <rdfs:label>days</rdfs:label>
    <rdfs:comment>Specifies the number of days noncurrent object versions expire.</rdfs:comment>
    <rdfs:domain rdf:resource="http://example.org/onto/class/yandex_storage_bucket"/>
    <rdfs:range rdf:resource="http://www.w3.org/2001/XMLSchema#string"/>
  </owl:DatatypeProperty>
  <owl:DatatypeProperty rdf:about="http://example.org/onto/prop/yandex_storage_bucket_days">
    <rdfs:label>days</rdfs:label>
    <rdfs:comment>Specifies the number of days noncurrent object versions transition.</rdfs:comment>
    <rdfs:domain rdf:resource="http://example.org/onto/class/yandex_storage_bucket"/>
    <rdfs:range rdf:resource="http://www.w3.org/2001/XMLSchema#string"/>
  </owl:DatatypeProperty>
  <owl:DatatypeProperty rdf:about="http://example.org/onto/prop/yandex_storage_bucket_storage_class">
    <rdfs:label>storage_class</rdfs:label>
    <rdfs:comment>Specifies the storage class to which you want the noncurrent object versions to transition. Supported values: [`STANDARD_IA`, `COLD`, `ICE`].</rdfs:comment>
    <rdfs:domain rdf:resource="http://example.org/onto/class/yandex_storage_bucket"/>
    <rdfs:range rdf:resource="http://www.w3.org/2001/XMLSchema#string"/>
  </owl:DatatypeProperty>
  <owl:DatatypeProperty rdf:about="http://example.org/onto/prop/yandex_storage_bucket_date">
    <rdfs:label>date</rdfs:label>
    <rdfs:comment>Specifies the date after which you want the corresponding action to take effect.</rdfs:comment>
    <rdfs:domain rdf:resource="http://example.org/onto/class/yandex_storage_bucket"/>
    <rdfs:range rdf:resource="http://www.w3.org/2001/XMLSchema#string"/>
  </owl:DatatypeProperty>
  <owl:DatatypeProperty rdf:about="http://example.org/onto/prop/yandex_storage_bucket_days">
    <rdfs:label>days</rdfs:label>
    <rdfs:comment>Specifies the number of days after object creation when the specific rule action takes effect.</rdfs:comment>
    <rdfs:domain rdf:resource="http://example.org/onto/class/yandex_storage_bucket"/>
    <rdfs:range rdf:resource="http://www.w3.org/2001/XMLSchema#string"/>
  </owl:DatatypeProperty>
  <owl:DatatypeProperty rdf:about="http://example.org/onto/prop/yandex_storage_bucket_storage_class">
    <rdfs:label>storage_class</rdfs:label>
    <rdfs:comment>Specifies the storage class to which you want the object to transition. Supported values: [`STANDARD_IA`, `COLD`, `ICE`].</rdfs:comment>
    <rdfs:domain rdf:resource="http://example.org/onto/class/yandex_storage_bucket"/>
    <rdfs:range rdf:resource="http://www.w3.org/2001/XMLSchema#string"/>
  </owl:DatatypeProperty>
  <owl:DatatypeProperty rdf:about="http://example.org/onto/prop/yandex_storage_bucket_target_bucket">
    <rdfs:label>target_bucket</rdfs:label>
    <rdfs:comment>The name of the bucket that will receive the log objects.</rdfs:comment>
    <rdfs:domain rdf:resource="http://example.org/onto/class/yandex_storage_bucket"/>
    <rdfs:range rdf:resource="http://www.w3.org/2001/XMLSchema#string"/>
  </owl:DatatypeProperty>
  <owl:DatatypeProperty rdf:about="http://example.org/onto/prop/yandex_storage_bucket_target_prefix">
    <rdfs:label>target_prefix</rdfs:label>
    <rdfs:comment>To specify a key prefix for log objects.</rdfs:comment>
    <rdfs:domain rdf:resource="http://example.org/onto/class/yandex_storage_bucket"/>
    <rdfs:range rdf:resource="http://www.w3.org/2001/XMLSchema#string"/>
  </owl:DatatypeProperty>
  <owl:DatatypeProperty rdf:about="http://example.org/onto/prop/yandex_storage_bucket_object_lock_enabled">
    <rdfs:label>object_lock_enabled</rdfs:label>
    <rdfs:comment>Enable object locking in a bucket. Require versioning to be enabled.</rdfs:comment>
    <rdfs:domain rdf:resource="http://example.org/onto/class/yandex_storage_bucket"/>
    <rdfs:range rdf:resource="http://www.w3.org/2001/XMLSchema#string"/>
  </owl:DatatypeProperty>
  <owl:DatatypeProperty rdf:about="http://example.org/onto/prop/yandex_storage_bucket_days">
    <rdfs:label>days</rdfs:label>
    <rdfs:comment>Specifies a retention period in days after uploading an object version. It must be a positive integer. You can't set it simultaneously with `years`.</rdfs:comment>
    <rdfs:domain rdf:resource="http://example.org/onto/class/yandex_storage_bucket"/>
    <rdfs:range rdf:resource="http://www.w3.org/2001/XMLSchema#string"/>
  </owl:DatatypeProperty>
  <owl:DatatypeProperty rdf:about="http://example.org/onto/prop/yandex_storage_bucket_mode">
    <rdfs:label>mode</rdfs:label>
    <rdfs:comment>Specifies a type of object lock. One of `["GOVERNANCE", "COMPLIANCE"]`.</rdfs:comment>
    <rdfs:domain rdf:resource="http://example.org/onto/class/yandex_storage_bucket"/>
    <rdfs:range rdf:resource="http://www.w3.org/2001/XMLSchema#string"/>
  </owl:DatatypeProperty>
  <owl:DatatypeProperty rdf:about="http://example.org/onto/prop/yandex_storage_bucket_years">
    <rdfs:label>years</rdfs:label>
    <rdfs:comment>Specifies a retention period in years after uploading an object version. It must be a positive integer. You can't set it simultaneously with `days`.</rdfs:comment>
    <rdfs:domain rdf:resource="http://example.org/onto/class/yandex_storage_bucket"/>
    <rdfs:range rdf:resource="http://www.w3.org/2001/XMLSchema#string"/>
  </owl:DatatypeProperty>
  <owl:DatatypeProperty rdf:about="http://example.org/onto/prop/yandex_storage_bucket_kms_master_key_id">
    <rdfs:label>kms_master_key_id</rdfs:label>
    <rdfs:comment>The KMS master key ID used for the SSE-KMS encryption.</rdfs:comment>
    <rdfs:domain rdf:resource="http://example.org/onto/class/yandex_storage_bucket"/>
    <rdfs:range rdf:resource="http://www.w3.org/2001/XMLSchema#string"/>
  </owl:DatatypeProperty>
  <owl:DatatypeProperty rdf:about="http://example.org/onto/prop/yandex_storage_bucket_sse_algorithm">
    <rdfs:label>sse_algorithm</rdfs:label>
    <rdfs:comment>The server-side encryption algorithm to use. Single valid value is `aws:kms`.</rdfs:comment>
    <rdfs:domain rdf:resource="http://example.org/onto/class/yandex_storage_bucket"/>
    <rdfs:range rdf:resource="http://www.w3.org/2001/XMLSchema#string"/>
  </owl:DatatypeProperty>
  <owl:DatatypeProperty rdf:about="http://example.org/onto/prop/yandex_storage_bucket_enabled">
    <rdfs:label>enabled</rdfs:label>
    <rdfs:comment>Enable versioning. Once you version-enable a bucket, it can never return to an unversioned state. You can, however, suspend versioning on that bucket.</rdfs:comment>
    <rdfs:domain rdf:resource="http://example.org/onto/class/yandex_storage_bucket"/>
    <rdfs:range rdf:resource="http://www.w3.org/2001/XMLSchema#string"/>
  </owl:DatatypeProperty>
  <owl:DatatypeProperty rdf:about="http://example.org/onto/prop/yandex_storage_bucket_error_document">
    <rdfs:label>error_document</rdfs:label>
    <rdfs:comment>An absolute path to the document to return in case of a 4XX error.</rdfs:comment>
    <rdfs:domain rdf:resource="http://example.org/onto/class/yandex_storage_bucket"/>
    <rdfs:range rdf:resource="http://www.w3.org/2001/XMLSchema#string"/>
  </owl:DatatypeProperty>
  <owl:DatatypeProperty rdf:about="http://example.org/onto/prop/yandex_storage_bucket_index_document">
    <rdfs:label>index_document</rdfs:label>
    <rdfs:comment>Storage returns this index document when requests are made to the root domain or any of the subfolders (unless using `redirect_all_requests_to`).</rdfs:comment>
    <rdfs:domain rdf:resource="http://example.org/onto/class/yandex_storage_bucket"/>
    <rdfs:range rdf:resource="http://www.w3.org/2001/XMLSchema#string"/>
  </owl:DatatypeProperty>
  <owl:DatatypeProperty rdf:about="http://example.org/onto/prop/yandex_storage_bucket_redirect_all_requests_to">
    <rdfs:label>redirect_all_requests_to</rdfs:label>
    <rdfs:comment>A hostname to redirect all website requests for this bucket to. Hostname can optionally be prefixed with a protocol (`http://` or `https://`) to use when redirecting requests. The default is the protocol that is used in the original request.</rdfs:comment>
    <rdfs:domain rdf:resource="http://example.org/onto/class/yandex_storage_bucket"/>
    <rdfs:range rdf:resource="http://www.w3.org/2001/XMLSchema#string"/>
  </owl:DatatypeProperty>
  <owl:DatatypeProperty rdf:about="http://example.org/onto/prop/yandex_storage_bucket_routing_rules">
    <rdfs:label>routing_rules</rdfs:label>
    <rdfs:comment>A JSON array containing [routing rules](https://yandex.cloud/docs/storage/s3/api-ref/hosting/upload#request-scheme) describing redirect behavior and when redirects are applied.</rdfs:comment>
    <rdfs:domain rdf:resource="http://example.org/onto/class/yandex_storage_bucket"/>
    <rdfs:range rdf:resource="http://www.w3.org/2001/XMLSchema#string"/>
  </owl:DatatypeProperty>
</rdf:RDF>
