<?xml version="1.0" encoding="UTF-8"?>
<rdf:RDF
  xmlns:rdf="http://www.w3.org/1999/02/22-rdf-syntax-ns#"
  xmlns:rdfs="http://www.w3.org/2000/01/rdf-schema#"
  xmlns:owl="http://www.w3.org/2002/07/owl#"
  xmlns:xsd="http://www.w3.org/2001/XMLSchema#"
  xml:base="http://example.org/onto/">
  <owl:Class rdf:about="http://example.org/onto/class/yandex_kms_symmetric_key">
    <rdfs:label>yandex_kms_symmetric_key</rdfs:label>
    <rdfs:comment>A symmetric KMS key that may contain several versions of the cryptographic material.</rdfs:comment>
  </owl:Class>
  <owl:DatatypeProperty rdf:about="http://example.org/onto/prop/yandex_kms_symmetric_key_created_at">
    <rdfs:label>created_at</rdfs:label>
    <rdfs:comment>Time when the key was created.</rdfs:comment>
    <rdfs:domain rdf:resource="http://example.org/onto/class/yandex_kms_symmetric_key"/>
    <rdfs:range rdf:resource="http://www.w3.org/2001/XMLSchema#string"/>
  </owl:DatatypeProperty>
  <owl:DatatypeProperty rdf:about="http://example.org/onto/prop/yandex_kms_symmetric_key_default_algorithm">
    <rdfs:label>default_algorithm</rdfs:label>
    <rdfs:comment>Default encryption algorithm to be used with new versions of the key.</rdfs:comment>
    <rdfs:domain rdf:resource="http://example.org/onto/class/yandex_kms_symmetric_key"/>
    <rdfs:range rdf:resource="http://www.w3.org/2001/XMLSchema#string"/>
  </owl:DatatypeProperty>
  <owl:DatatypeProperty rdf:about="http://example.org/onto/prop/yandex_kms_symmetric_key_deletion_protection">
    <rdfs:label>deletion_protection</rdfs:label>
    <rdfs:comment>Flag that inhibits deletion of the key</rdfs:comment>
    <rdfs:domain rdf:resource="http://example.org/onto/class/yandex_kms_symmetric_key"/>
    <rdfs:range rdf:resource="http://www.w3.org/2001/XMLSchema#string"/>
  </owl:DatatypeProperty>
  <owl:DatatypeProperty rdf:about="http://example.org/onto/prop/yandex_kms_symmetric_key_description">
    <rdfs:label>description</rdfs:label>
    <rdfs:comment>Description of the key.</rdfs:comment>
    <rdfs:domain rdf:resource="http://example.org/onto/class/yandex_kms_symmetric_key"/>
    <rdfs:range rdf:resource="http://www.w3.org/2001/XMLSchema#string"/>
  </owl:DatatypeProperty>
  <owl:DatatypeProperty rdf:about="http://example.org/onto/prop/yandex_kms_symmetric_key_folder_id">
    <rdfs:label>folder_id</rdfs:label>
    <rdfs:comment>ID of the folder that the key belongs to.</rdfs:comment>
    <rdfs:domain rdf:resource="http://example.org/onto/class/yandex_kms_symmetric_key"/>
    <rdfs:range rdf:resource="http://www.w3.org/2001/XMLSchema#string"/>
  </owl:DatatypeProperty>
  <owl:DatatypeProperty rdf:about="http://example.org/onto/prop/yandex_kms_symmetric_key_id">
    <rdfs:label>id</rdfs:label>
    <rdfs:comment>ID of the symmetric KMS key to return.
 To get the ID of a symmetric KMS key use a [SymmetricKeyService.List] request.</rdfs:comment>
    <rdfs:domain rdf:resource="http://example.org/onto/class/yandex_kms_symmetric_key"/>
    <rdfs:range rdf:resource="http://www.w3.org/2001/XMLSchema#string"/>
  </owl:DatatypeProperty>
  <owl:DatatypeProperty rdf:about="http://example.org/onto/prop/yandex_kms_symmetric_key_labels">
    <rdfs:label>labels</rdfs:label>
    <rdfs:comment>Custom labels for the key as `key:value` pairs. Maximum 64 per key.</rdfs:comment>
    <rdfs:domain rdf:resource="http://example.org/onto/class/yandex_kms_symmetric_key"/>
    <rdfs:range rdf:resource="http://www.w3.org/2001/XMLSchema#string"/>
  </owl:DatatypeProperty>
  <owl:DatatypeProperty rdf:about="http://example.org/onto/prop/yandex_kms_symmetric_key_name">
    <rdfs:label>name</rdfs:label>
    <rdfs:comment>Name of the key.</rdfs:comment>
    <rdfs:domain rdf:resource="http://example.org/onto/class/yandex_kms_symmetric_key"/>
    <rdfs:range rdf:resource="http://www.w3.org/2001/XMLSchema#string"/>
  </owl:DatatypeProperty>
  <owl:DatatypeProperty rdf:about="http://example.org/onto/prop/yandex_kms_symmetric_key_rotated_at">
    <rdfs:label>rotated_at</rdfs:label>
    <rdfs:comment>Time of the last key rotation (time when the last version was created).
 Empty if the key does not have versions yet.</rdfs:comment>
    <rdfs:domain rdf:resource="http://example.org/onto/class/yandex_kms_symmetric_key"/>
    <rdfs:range rdf:resource="http://www.w3.org/2001/XMLSchema#string"/>
  </owl:DatatypeProperty>
  <owl:DatatypeProperty rdf:about="http://example.org/onto/prop/yandex_kms_symmetric_key_rotation_period">
    <rdfs:label>rotation_period</rdfs:label>
    <rdfs:comment>Time period between automatic key rotations.</rdfs:comment>
    <rdfs:domain rdf:resource="http://example.org/onto/class/yandex_kms_symmetric_key"/>
    <rdfs:range rdf:resource="http://www.w3.org/2001/XMLSchema#string"/>
  </owl:DatatypeProperty>
  <owl:DatatypeProperty rdf:about="http://example.org/onto/prop/yandex_kms_symmetric_key_status">
    <rdfs:label>status</rdfs:label>
    <rdfs:comment>Current status of the key.</rdfs:comment>
    <rdfs:domain rdf:resource="http://example.org/onto/class/yandex_kms_symmetric_key"/>
    <rdfs:range rdf:resource="http://www.w3.org/2001/XMLSchema#string"/>
  </owl:DatatypeProperty>
  <owl:DatatypeProperty rdf:about="http://example.org/onto/prop/yandex_kms_symmetric_key_symmetric_key_id">
    <rdfs:label>symmetric_key_id</rdfs:label>
    <rdfs:comment>ID of the symmetric KMS key to return.
 To get the ID of a symmetric KMS key use a [SymmetricKeyService.List] request.</rdfs:comment>
    <rdfs:domain rdf:resource="http://example.org/onto/class/yandex_kms_symmetric_key"/>
    <rdfs:range rdf:resource="http://www.w3.org/2001/XMLSchema#string"/>
  </owl:DatatypeProperty>
  <owl:DatatypeProperty rdf:about="http://example.org/onto/prop/yandex_kms_symmetric_key_create">
    <rdfs:label>create</rdfs:label>
    <rdfs:comment>A string that can be [parsed as a duration](https://pkg.go.dev/time#ParseDuration) consisting of numbers and unit suffixes, such as "30s" or "2h45m". Valid time units are "s" (seconds), "m" (minutes), "h" (hours).</rdfs:comment>
    <rdfs:domain rdf:resource="http://example.org/onto/class/yandex_kms_symmetric_key"/>
    <rdfs:range rdf:resource="http://www.w3.org/2001/XMLSchema#string"/>
  </owl:DatatypeProperty>
  <owl:DatatypeProperty rdf:about="http://example.org/onto/prop/yandex_kms_symmetric_key_delete">
    <rdfs:label>delete</rdfs:label>
    <rdfs:comment>A string that can be [parsed as a duration](https://pkg.go.dev/time#ParseDuration) consisting of numbers and unit suffixes, such as "30s" or "2h45m". Valid time units are "s" (seconds), "m" (minutes), "h" (hours). Setting a timeout for a Delete operation is only applicable if changes are saved into state before the destroy operation occurs.</rdfs:comment>
    <rdfs:domain rdf:resource="http://example.org/onto/class/yandex_kms_symmetric_key"/>
    <rdfs:range rdf:resource="http://www.w3.org/2001/XMLSchema#string"/>
  </owl:DatatypeProperty>
  <owl:DatatypeProperty rdf:about="http://example.org/onto/prop/yandex_kms_symmetric_key_read">
    <rdfs:label>read</rdfs:label>
    <rdfs:comment>A string that can be [parsed as a duration](https://pkg.go.dev/time#ParseDuration) consisting of numbers and unit suffixes, such as "30s" or "2h45m". Valid time units are "s" (seconds), "m" (minutes), "h" (hours). Read operations occur during any refresh or planning operation when refresh is enabled.</rdfs:comment>
    <rdfs:domain rdf:resource="http://example.org/onto/class/yandex_kms_symmetric_key"/>
    <rdfs:range rdf:resource="http://www.w3.org/2001/XMLSchema#string"/>
  </owl:DatatypeProperty>
  <owl:DatatypeProperty rdf:about="http://example.org/onto/prop/yandex_kms_symmetric_key_update">
    <rdfs:label>update</rdfs:label>
    <rdfs:comment>A string that can be [parsed as a duration](https://pkg.go.dev/time#ParseDuration) consisting of numbers and unit suffixes, such as "30s" or "2h45m". Valid time units are "s" (seconds), "m" (minutes), "h" (hours).</rdfs:comment>
    <rdfs:domain rdf:resource="http://example.org/onto/class/yandex_kms_symmetric_key"/>
    <rdfs:range rdf:resource="http://www.w3.org/2001/XMLSchema#string"/>
  </owl:DatatypeProperty>
</rdf:RDF>
