<?xml version="1.0" encoding="UTF-8"?>
<rdf:RDF
  xmlns:rdf="http://www.w3.org/1999/02/22-rdf-syntax-ns#"
  xmlns:rdfs="http://www.w3.org/2000/01/rdf-schema#"
  xmlns:owl="http://www.w3.org/2002/07/owl#"
  xmlns:xsd="http://www.w3.org/2001/XMLSchema#"
  xml:base="http://example.org/onto/">
  <owl:Class rdf:about="http://example.org/onto/class/yandex_cloudregistry_registry">
    <rdfs:label>yandex_cloudregistry_registry</rdfs:label>
    <rdfs:comment>A Registry resource. For more information, see the [Registry](/docs/cloud-registry/concepts/registry) section of the documentation.</rdfs:comment>
  </owl:Class>
  <owl:DatatypeProperty rdf:about="http://example.org/onto/prop/yandex_cloudregistry_registry_created_at">
    <rdfs:label>created_at</rdfs:label>
    <rdfs:comment>Output only. Creation timestamp in [RFC3339](https://www.ietf.org/rfc/rfc3339.txt) text format.</rdfs:comment>
    <rdfs:domain rdf:resource="http://example.org/onto/class/yandex_cloudregistry_registry"/>
    <rdfs:range rdf:resource="http://www.w3.org/2001/XMLSchema#string"/>
  </owl:DatatypeProperty>
  <owl:DatatypeProperty rdf:about="http://example.org/onto/prop/yandex_cloudregistry_registry_description">
    <rdfs:label>description</rdfs:label>
    <rdfs:comment>Description of the registry.</rdfs:comment>
    <rdfs:domain rdf:resource="http://example.org/onto/class/yandex_cloudregistry_registry"/>
    <rdfs:range rdf:resource="http://www.w3.org/2001/XMLSchema#string"/>
  </owl:DatatypeProperty>
  <owl:DatatypeProperty rdf:about="http://example.org/onto/prop/yandex_cloudregistry_registry_folder_id">
    <rdfs:label>folder_id</rdfs:label>
    <rdfs:comment>ID of the folder that the registry belongs to.</rdfs:comment>
    <rdfs:domain rdf:resource="http://example.org/onto/class/yandex_cloudregistry_registry"/>
    <rdfs:range rdf:resource="http://www.w3.org/2001/XMLSchema#string"/>
  </owl:DatatypeProperty>
  <owl:DatatypeProperty rdf:about="http://example.org/onto/prop/yandex_cloudregistry_registry_id">
    <rdfs:label>id</rdfs:label>
    <rdfs:comment>ID of the Registry resource to return.

 To get the registry ID use a [RegistryService.List] request.</rdfs:comment>
    <rdfs:domain rdf:resource="http://example.org/onto/class/yandex_cloudregistry_registry"/>
    <rdfs:range rdf:resource="http://www.w3.org/2001/XMLSchema#string"/>
  </owl:DatatypeProperty>
  <owl:DatatypeProperty rdf:about="http://example.org/onto/prop/yandex_cloudregistry_registry_kind">
    <rdfs:label>kind</rdfs:label>
    <rdfs:comment>Kind of the registry.</rdfs:comment>
    <rdfs:domain rdf:resource="http://example.org/onto/class/yandex_cloudregistry_registry"/>
    <rdfs:range rdf:resource="http://www.w3.org/2001/XMLSchema#string"/>
  </owl:DatatypeProperty>
  <owl:DatatypeProperty rdf:about="http://example.org/onto/prop/yandex_cloudregistry_registry_labels">
    <rdfs:label>labels</rdfs:label>
    <rdfs:comment>Resource labels as `key:value` pairs. Maximum of 64 per resource.</rdfs:comment>
    <rdfs:domain rdf:resource="http://example.org/onto/class/yandex_cloudregistry_registry"/>
    <rdfs:range rdf:resource="http://www.w3.org/2001/XMLSchema#string"/>
  </owl:DatatypeProperty>
  <owl:DatatypeProperty rdf:about="http://example.org/onto/prop/yandex_cloudregistry_registry_modified_at">
    <rdfs:label>modified_at</rdfs:label>
    <rdfs:comment>Output only. Modification timestamp in [RFC3339](https://www.ietf.org/rfc/rfc3339.txt) text format.</rdfs:comment>
    <rdfs:domain rdf:resource="http://example.org/onto/class/yandex_cloudregistry_registry"/>
    <rdfs:range rdf:resource="http://www.w3.org/2001/XMLSchema#string"/>
  </owl:DatatypeProperty>
  <owl:DatatypeProperty rdf:about="http://example.org/onto/prop/yandex_cloudregistry_registry_name">
    <rdfs:label>name</rdfs:label>
    <rdfs:comment>Name of the registry.</rdfs:comment>
    <rdfs:domain rdf:resource="http://example.org/onto/class/yandex_cloudregistry_registry"/>
    <rdfs:range rdf:resource="http://www.w3.org/2001/XMLSchema#string"/>
  </owl:DatatypeProperty>
  <owl:DatatypeProperty rdf:about="http://example.org/onto/prop/yandex_cloudregistry_registry_properties">
    <rdfs:label>properties</rdfs:label>
    <rdfs:comment>Resource properties as `key:value` pairs. Maximum of 64 per resource.</rdfs:comment>
    <rdfs:domain rdf:resource="http://example.org/onto/class/yandex_cloudregistry_registry"/>
    <rdfs:range rdf:resource="http://www.w3.org/2001/XMLSchema#string"/>
  </owl:DatatypeProperty>
  <owl:DatatypeProperty rdf:about="http://example.org/onto/prop/yandex_cloudregistry_registry_registry_id">
    <rdfs:label>registry_id</rdfs:label>
    <rdfs:comment>ID of the Registry resource to return.

 To get the registry ID use a [RegistryService.List] request.</rdfs:comment>
    <rdfs:domain rdf:resource="http://example.org/onto/class/yandex_cloudregistry_registry"/>
    <rdfs:range rdf:resource="http://www.w3.org/2001/XMLSchema#string"/>
  </owl:DatatypeProperty>
  <owl:DatatypeProperty rdf:about="http://example.org/onto/prop/yandex_cloudregistry_registry_status">
    <rdfs:label>status</rdfs:label>
    <rdfs:comment>Output only. Status of the registry.</rdfs:comment>
    <rdfs:domain rdf:resource="http://example.org/onto/class/yandex_cloudregistry_registry"/>
    <rdfs:range rdf:resource="http://www.w3.org/2001/XMLSchema#string"/>
  </owl:DatatypeProperty>
  <owl:DatatypeProperty rdf:about="http://example.org/onto/prop/yandex_cloudregistry_registry_timeouts">
    <rdfs:label>timeouts</rdfs:label>
    <rdfs:domain rdf:resource="http://example.org/onto/class/yandex_cloudregistry_registry"/>
    <rdfs:range rdf:resource="http://www.w3.org/2001/XMLSchema#string"/>
  </owl:DatatypeProperty>
  <owl:DatatypeProperty rdf:about="http://example.org/onto/prop/yandex_cloudregistry_registry_type">
    <rdfs:label>type</rdfs:label>
    <rdfs:comment>Type of the registry.</rdfs:comment>
    <rdfs:domain rdf:resource="http://example.org/onto/class/yandex_cloudregistry_registry"/>
    <rdfs:range rdf:resource="http://www.w3.org/2001/XMLSchema#string"/>
  </owl:DatatypeProperty>
</rdf:RDF>
